<?xml version="1.0"?>
<rdf:RDF xmlns="http://purl.obolibrary.org/obo/gaz/subsets/oceans_and_seas/Southern_Ocean.owl#"
     xml:base="http://purl.obolibrary.org/obo/gaz/subsets/oceans_and_seas/Southern_Ocean.owl"
     xmlns:obo="http://purl.obolibrary.org/obo/"
     xmlns:owl="http://www.w3.org/2002/07/owl#"
     xmlns:rdf="http://www.w3.org/1999/02/22-rdf-syntax-ns#"
     xmlns:xml="http://www.w3.org/XML/1998/namespace"
     xmlns:xsd="http://www.w3.org/2001/XMLSchema#"
     xmlns:rdfs="http://www.w3.org/2000/01/rdf-schema#"
     xmlns:oboInOwl="http://www.geneontology.org/formats/oboInOwl#">
    <owl:Ontology rdf:about="http://purl.obolibrary.org/obo/gaz/subsets/oceans_and_seas/Southern_Ocean.owl">
        <owl:imports rdf:resource="http://purl.obolibrary.org/obo/gaz/imports/envo_import.owl"/>
        <owl:imports rdf:resource="http://purl.obolibrary.org/obo/gaz/imports/ro_import.owl"/>
    </owl:Ontology>
    


    <!-- 
    ///////////////////////////////////////////////////////////////////////////////////////
    //
    // Annotation properties
    //
    ///////////////////////////////////////////////////////////////////////////////////////
     -->

    


    <!-- http://purl.obolibrary.org/obo/IAO_0000115 -->

    <owl:AnnotationProperty rdf:about="http://purl.obolibrary.org/obo/IAO_0000115"/>
    


    <!-- http://www.geneontology.org/formats/oboInOwl#hasOBONamespace -->

    <owl:AnnotationProperty rdf:about="http://www.geneontology.org/formats/oboInOwl#hasOBONamespace"/>
    


    <!-- http://www.geneontology.org/formats/oboInOwl#id -->

    <owl:AnnotationProperty rdf:about="http://www.geneontology.org/formats/oboInOwl#id"/>
    


    <!-- 
    ///////////////////////////////////////////////////////////////////////////////////////
    //
    // Object Properties
    //
    ///////////////////////////////////////////////////////////////////////////////////////
     -->

    


    <!-- http://purl.obolibrary.org/obo/RO_0001025 -->

    <owl:ObjectProperty rdf:about="http://purl.obolibrary.org/obo/RO_0001025"/>
    


    <!-- 
    ///////////////////////////////////////////////////////////////////////////////////////
    //
    // Classes
    //
    ///////////////////////////////////////////////////////////////////////////////////////
     -->

    


    <!-- http://purl.obolibrary.org/obo/ENVO_00000016 -->

    <owl:Class rdf:about="http://purl.obolibrary.org/obo/ENVO_00000016"/>
    


    <!-- http://purl.obolibrary.org/obo/ENVO_00000029 -->

    <owl:Class rdf:about="http://purl.obolibrary.org/obo/ENVO_00000029"/>
    


    <!-- http://purl.obolibrary.org/obo/ENVO_00000032 -->

    <owl:Class rdf:about="http://purl.obolibrary.org/obo/ENVO_00000032"/>
    


    <!-- http://purl.obolibrary.org/obo/ENVO_00000084 -->

    <owl:Class rdf:about="http://purl.obolibrary.org/obo/ENVO_00000084"/>
    


    <!-- http://purl.obolibrary.org/obo/ENVO_00000100 -->

    <owl:Class rdf:about="http://purl.obolibrary.org/obo/ENVO_00000100"/>
    


    <!-- http://purl.obolibrary.org/obo/ENVO_00000106 -->

    <owl:Class rdf:about="http://purl.obolibrary.org/obo/ENVO_00000106"/>
    


    <!-- http://purl.obolibrary.org/obo/ENVO_00000167 -->

    <owl:Class rdf:about="http://purl.obolibrary.org/obo/ENVO_00000167"/>
    


    <!-- http://purl.obolibrary.org/obo/ENVO_00000220 -->

    <owl:Class rdf:about="http://purl.obolibrary.org/obo/ENVO_00000220"/>
    


    <!-- http://purl.obolibrary.org/obo/ENVO_00000222 -->

    <owl:Class rdf:about="http://purl.obolibrary.org/obo/ENVO_00000222"/>
    


    <!-- http://purl.obolibrary.org/obo/ENVO_00000275 -->

    <owl:Class rdf:about="http://purl.obolibrary.org/obo/ENVO_00000275"/>
    


    <!-- http://purl.obolibrary.org/obo/ENVO_00000305 -->

    <owl:Class rdf:about="http://purl.obolibrary.org/obo/ENVO_00000305"/>
    


    <!-- http://purl.obolibrary.org/obo/ENVO_00000398 -->

    <owl:Class rdf:about="http://purl.obolibrary.org/obo/ENVO_00000398"/>
    


    <!-- http://purl.obolibrary.org/obo/ENVO_00000475 -->

    <owl:Class rdf:about="http://purl.obolibrary.org/obo/ENVO_00000475"/>
    


    <!-- http://purl.obolibrary.org/obo/GAZ_00000373 -->

    <owl:Class rdf:about="http://purl.obolibrary.org/obo/GAZ_00000373"/>
    


    <!-- http://purl.obolibrary.org/obo/GAZ_00000375 -->

    <owl:Class rdf:about="http://purl.obolibrary.org/obo/GAZ_00000375">
        <rdfs:subClassOf rdf:resource="http://purl.obolibrary.org/obo/GAZ_01000004"/>
        <obo:IAO_0000115>A current in the Southern Ocean, that is not part of the west wind drift. The Antarctica shelf and the sea-bottom ridges cause turbulence in the water and the west wind drift may get weaker in such areas. This can be seen even at the ocean surface, reversing the normally observed easterly water movement.</obo:IAO_0000115>
        <oboInOwl:hasOBONamespace>GAZ</oboInOwl:hasOBONamespace>
        <oboInOwl:id>GAZ:00000375</oboInOwl:id>
        <rdfs:label>Weddell Gyre</rdfs:label>
    </owl:Class>
    


    <!-- http://purl.obolibrary.org/obo/GAZ_00000376 -->

    <owl:Class rdf:about="http://purl.obolibrary.org/obo/GAZ_00000376">
        <rdfs:subClassOf rdf:resource="http://purl.obolibrary.org/obo/GAZ_01000004"/>
        <obo:IAO_0000115>An ocean current that flows from west to east around Antarctica.</obo:IAO_0000115>
        <oboInOwl:hasOBONamespace>GAZ</oboInOwl:hasOBONamespace>
        <oboInOwl:id>GAZ:00000376</oboInOwl:id>
        <rdfs:label>Antarctic Circumpolar Current</rdfs:label>
    </owl:Class>
    


    <!-- http://purl.obolibrary.org/obo/GAZ_00014125 -->

    <owl:Class rdf:about="http://purl.obolibrary.org/obo/GAZ_00014125"/>
    


    <!-- http://purl.obolibrary.org/obo/GAZ_00014126 -->

    <owl:Class rdf:about="http://purl.obolibrary.org/obo/GAZ_00014126">
        <rdfs:subClassOf rdf:resource="http://purl.obolibrary.org/obo/GAZ_00014125"/>
        <oboInOwl:hasOBONamespace>GAZ</oboInOwl:hasOBONamespace>
        <oboInOwl:id>GAZ:00014126</oboInOwl:id>
        <rdfs:label>ANDEEP III station</rdfs:label>
    </owl:Class>
    


    <!-- http://purl.obolibrary.org/obo/GAZ_00014127 -->

    <owl:Class rdf:about="http://purl.obolibrary.org/obo/GAZ_00014127">
        <rdfs:subClassOf rdf:resource="http://purl.obolibrary.org/obo/GAZ_00014125"/>
        <oboInOwl:hasOBONamespace>GAZ</oboInOwl:hasOBONamespace>
        <oboInOwl:id>GAZ:00014127</oboInOwl:id>
        <rdfs:label>ANDEEP II station</rdfs:label>
    </owl:Class>
    


    <!-- http://purl.obolibrary.org/obo/GAZ_00014128 -->

    <owl:Class rdf:about="http://purl.obolibrary.org/obo/GAZ_00014128">
        <rdfs:subClassOf rdf:resource="http://purl.obolibrary.org/obo/GAZ_00014127"/>
        <oboInOwl:hasOBONamespace>GAZ</oboInOwl:hasOBONamespace>
        <oboInOwl:id>GAZ:00014128</oboInOwl:id>
        <rdfs:label>ANDEEP II, station 33</rdfs:label>
    </owl:Class>
    


    <!-- http://purl.obolibrary.org/obo/GAZ_00014129 -->

    <owl:Class rdf:about="http://purl.obolibrary.org/obo/GAZ_00014129">
        <rdfs:subClassOf rdf:resource="http://purl.obolibrary.org/obo/GAZ_00014126"/>
        <oboInOwl:hasOBONamespace>GAZ</oboInOwl:hasOBONamespace>
        <oboInOwl:id>GAZ:00014129</oboInOwl:id>
        <rdfs:label>ANDEEP III, station 59/7</rdfs:label>
    </owl:Class>
    


    <!-- http://purl.obolibrary.org/obo/GAZ_00014130 -->

    <owl:Class rdf:about="http://purl.obolibrary.org/obo/GAZ_00014130">
        <rdfs:subClassOf rdf:resource="http://purl.obolibrary.org/obo/GAZ_00014126"/>
        <oboInOwl:hasOBONamespace>GAZ</oboInOwl:hasOBONamespace>
        <oboInOwl:id>GAZ:00014130</oboInOwl:id>
        <rdfs:label>ANDEEP III, station 102/8</rdfs:label>
    </owl:Class>
    


    <!-- http://purl.obolibrary.org/obo/GAZ_01000004 -->

    <owl:Class rdf:about="http://purl.obolibrary.org/obo/GAZ_01000004"/>
    


    <!-- http://www.w3.org/2002/07/owl#NamedIndividual -->

    <owl:Class rdf:about="http://www.w3.org/2002/07/owl#NamedIndividual"/>
    


    <!-- 
    ///////////////////////////////////////////////////////////////////////////////////////
    //
    // Individuals
    //
    ///////////////////////////////////////////////////////////////////////////////////////
     -->

    


    <!-- http://purl.obolibrary.org/obo/GAZ_00000373 -->

    <owl:NamedIndividual rdf:about="http://purl.obolibrary.org/obo/GAZ_00000373"/>
    


    <!-- http://purl.obolibrary.org/obo/GAZ_00002624 -->

    <owl:NamedIndividual rdf:about="http://purl.obolibrary.org/obo/GAZ_00002624">
        <obo:RO_0001025 rdf:resource="http://purl.obolibrary.org/obo/GAZ_00141552"/>
        <obo:IAO_0000115>A strait between the Argentine Islands, Petermann Island and Hovgaard Island and the Graham Coast.</obo:IAO_0000115>
        <oboInOwl:hasOBONamespace>GAZ</oboInOwl:hasOBONamespace>
        <oboInOwl:id>GAZ:00002624</oboInOwl:id>
        <rdfs:label>Penola Strait</rdfs:label>
    </owl:NamedIndividual>
    


    <!-- http://purl.obolibrary.org/obo/GAZ_00002625 -->

    <owl:NamedIndividual rdf:about="http://purl.obolibrary.org/obo/GAZ_00002625">
        <obo:RO_0001025 rdf:resource="http://purl.obolibrary.org/obo/GAZ_00023304"/>
        <obo:IAO_0000115>A sound that extend about 55 km long and wide. The sound encompasses 4,000 km of shoreline which opens to the Ross Sea to the north. The Royal Society Range rises from sea level to 4,205 m on the western shoreline. The nearby McMurdo Ice Shelf scribes McMurdo Sound&apos;s southern boundary. Ross Island, an historic jumping-off point for polar explorers, designates the eastern boundary.</obo:IAO_0000115>
        <oboInOwl:hasOBONamespace>GAZ</oboInOwl:hasOBONamespace>
        <oboInOwl:id>GAZ:00002625</oboInOwl:id>
        <rdfs:label>McMurdo Sound</rdfs:label>
    </owl:NamedIndividual>
    


    <!-- http://purl.obolibrary.org/obo/GAZ_00003703 -->

    <owl:NamedIndividual rdf:about="http://purl.obolibrary.org/obo/GAZ_00003703">
        <obo:RO_0001025 rdf:resource="http://purl.obolibrary.org/obo/GAZ_00007475"/>
        <obo:IAO_0000115>A broad ice shelf at the head of Prydz Bay between the Lars Christensen Coast and Ingrid Christensen Coast It is part of Mac Robertson Land.</obo:IAO_0000115>
        <oboInOwl:hasOBONamespace>GAZ</oboInOwl:hasOBONamespace>
        <oboInOwl:id>GAZ:00003703</oboInOwl:id>
        <rdfs:label>Amery Ice Shelf</rdfs:label>
    </owl:NamedIndividual>
    


    <!-- http://purl.obolibrary.org/obo/GAZ_00003705 -->

    <owl:NamedIndividual rdf:about="http://purl.obolibrary.org/obo/GAZ_00003705">
        <obo:RO_0001025 rdf:resource="http://purl.obolibrary.org/obo/GAZ_00139422"/>
        <obo:IAO_0000115>A small island 0.25 mi NE of Turner Island, lying off Breidnes Peninsula, Vestfold Hills.</obo:IAO_0000115>
        <oboInOwl:hasOBONamespace>GAZ</oboInOwl:hasOBONamespace>
        <oboInOwl:id>GAZ:00003705</oboInOwl:id>
        <rdfs:label>Magnetic Island</rdfs:label>
    </owl:NamedIndividual>
    


    <!-- http://purl.obolibrary.org/obo/GAZ_00003918 -->

    <owl:NamedIndividual rdf:about="http://purl.obolibrary.org/obo/GAZ_00003918">
        <obo:RO_0001025 rdf:resource="http://purl.obolibrary.org/obo/GAZ_00141276"/>
        <oboInOwl:hasOBONamespace>GAZ</oboInOwl:hasOBONamespace>
        <oboInOwl:id>GAZ:00003918</oboInOwl:id>
        <rdfs:label>Showa Station</rdfs:label>
    </owl:NamedIndividual>
    


    <!-- http://purl.obolibrary.org/obo/GAZ_00004041 -->

    <owl:NamedIndividual rdf:about="http://purl.obolibrary.org/obo/GAZ_00004041">
        <obo:RO_0001025 rdf:resource="http://purl.obolibrary.org/obo/GAZ_00004045"/>
        <obo:IAO_0000115>A group of sub-antarctic islands, lying off the northeastern tip of the Antarctic Peninsula, from which Joinville Island group is separated by the Antarctic Sound.</obo:IAO_0000115>
        <oboInOwl:hasOBONamespace>GAZ</oboInOwl:hasOBONamespace>
        <oboInOwl:id>GAZ:00004041</oboInOwl:id>
        <rdfs:label>Joinville Island Group</rdfs:label>
    </owl:NamedIndividual>
    


    <!-- http://purl.obolibrary.org/obo/GAZ_00004042 -->

    <owl:NamedIndividual rdf:about="http://purl.obolibrary.org/obo/GAZ_00004042">
        <obo:RO_0001025 rdf:resource="http://purl.obolibrary.org/obo/GAZ_00004041"/>
        <obo:IAO_0000115>An ice-covered island lying E of the NE tip of Antarctic Peninsula and S of Joinville Island.</obo:IAO_0000115>
        <oboInOwl:hasOBONamespace>GAZ</oboInOwl:hasOBONamespace>
        <oboInOwl:id>GAZ:00004042</oboInOwl:id>
        <rdfs:label>Dundee Island</rdfs:label>
    </owl:NamedIndividual>
    


    <!-- http://purl.obolibrary.org/obo/GAZ_00004043 -->

    <owl:NamedIndividual rdf:about="http://purl.obolibrary.org/obo/GAZ_00004043">
        <obo:RO_0001025 rdf:resource="http://purl.obolibrary.org/obo/GAZ_00004041"/>
        <obo:IAO_0000115>The northernmost island of the Joinville Island group, 17 mi long, lying immediately N of Joinville Island, from which it is separated by Larsen Channel.</obo:IAO_0000115>
        <oboInOwl:hasOBONamespace>GAZ</oboInOwl:hasOBONamespace>
        <oboInOwl:id>GAZ:00004043</oboInOwl:id>
        <rdfs:label>D&apos;Urville Island</rdfs:label>
    </owl:NamedIndividual>
    


    <!-- http://purl.obolibrary.org/obo/GAZ_00004044 -->

    <owl:NamedIndividual rdf:about="http://purl.obolibrary.org/obo/GAZ_00004044">
        <obo:RO_0001025 rdf:resource="http://purl.obolibrary.org/obo/GAZ_00004041"/>
        <obo:IAO_0000115>The largest island of the Joinville Island group, about 40 mi long in an E-W direction and 12 mi wide, lying off the NE tip of Antarctic Peninsula, from which it is separated by Antarctic Sound.</obo:IAO_0000115>
        <oboInOwl:hasOBONamespace>GAZ</oboInOwl:hasOBONamespace>
        <oboInOwl:id>GAZ:00004044</oboInOwl:id>
        <rdfs:label>Joinville Island</rdfs:label>
    </owl:NamedIndividual>
    


    <!-- http://purl.obolibrary.org/obo/GAZ_00004045 -->

    <owl:NamedIndividual rdf:about="http://purl.obolibrary.org/obo/GAZ_00004045">
        <obo:RO_0001025 rdf:resource="http://purl.obolibrary.org/obo/GAZ_00000373"/>
        <obo:IAO_0000115>A sea defined by the bay formed from the coasts of Coats Land and the Antarctic Peninsula. Much of the southern part of the sea, up to Elephant Island, is permanent ice, the Filchner-Ronne Ice Shelf. Its W limit is the tip of the Antarctic Peninsula at 65degW and its E limit Cape Norvegica at 12degW.</obo:IAO_0000115>
        <oboInOwl:hasOBONamespace>GAZ</oboInOwl:hasOBONamespace>
        <oboInOwl:id>GAZ:00004045</oboInOwl:id>
        <rdfs:label>Weddell Sea</rdfs:label>
    </owl:NamedIndividual>
    


    <!-- http://purl.obolibrary.org/obo/GAZ_00004047 -->

    <owl:NamedIndividual rdf:about="http://purl.obolibrary.org/obo/GAZ_00004047">
        <obo:RO_0001025 rdf:resource="http://purl.obolibrary.org/obo/GAZ_00141552"/>
        <obo:IAO_0000115>A strait separating the Palmer Archipelago from the Antarctic Peninsula.</obo:IAO_0000115>
        <oboInOwl:hasOBONamespace>GAZ</oboInOwl:hasOBONamespace>
        <oboInOwl:id>GAZ:00004047</oboInOwl:id>
        <rdfs:label>Gerlache Strait</rdfs:label>
    </owl:NamedIndividual>
    


    <!-- http://purl.obolibrary.org/obo/GAZ_00004057 -->

    <owl:NamedIndividual rdf:about="http://purl.obolibrary.org/obo/GAZ_00004057">
        <obo:RO_0001025 rdf:resource="http://purl.obolibrary.org/obo/GAZ_00014096"/>
        <obo:IAO_0000115>An island lying on the E side of McMurdo Sound and extending 43 mi from Cape Bird on the N to Cape Armitage on the S, and a like distance from Cape Royds on the W to Cape Crozier on the east This island is entirely volcanic, Mount Erebus, 3,795 m, near the center, being an active volcano; and Mount Terror, 3,230 m, about 20 mi eastward, being an extinct volcano. Mount Bird rises to 1,765 m just S of Cape Bird.</obo:IAO_0000115>
        <oboInOwl:hasOBONamespace>GAZ</oboInOwl:hasOBONamespace>
        <oboInOwl:id>GAZ:00004057</oboInOwl:id>
        <rdfs:label>Ross Island</rdfs:label>
    </owl:NamedIndividual>
    


    <!-- http://purl.obolibrary.org/obo/GAZ_00004244 -->

    <owl:NamedIndividual rdf:about="http://purl.obolibrary.org/obo/GAZ_00004244">
        <obo:RO_0001025 rdf:resource="http://purl.obolibrary.org/obo/GAZ_00023358"/>
        <obo:IAO_0000115>An American Antarctic research center located on the southern tip of Ross Island on the shore of McMurdo Sound.</obo:IAO_0000115>
        <oboInOwl:hasOBONamespace>GAZ</oboInOwl:hasOBONamespace>
        <oboInOwl:id>GAZ:00004244</oboInOwl:id>
        <rdfs:label>McMurdo Station</rdfs:label>
    </owl:NamedIndividual>
    


    <!-- http://purl.obolibrary.org/obo/GAZ_00004380 -->

    <owl:NamedIndividual rdf:about="http://purl.obolibrary.org/obo/GAZ_00004380">
        <obo:RO_0001025 rdf:resource="http://purl.obolibrary.org/obo/GAZ_00141552"/>
        <obo:IAO_0000115>A group of islands extending from Tower Island in the N to Anvers Island in the S, lying NW of Antarctic Peninsula, from which it is separated by Gerlache Strait.</obo:IAO_0000115>
        <oboInOwl:hasOBONamespace>GAZ</oboInOwl:hasOBONamespace>
        <oboInOwl:id>GAZ:00004380</oboInOwl:id>
        <rdfs:label>Palmer Archipelago</rdfs:label>
    </owl:NamedIndividual>
    


    <!-- http://purl.obolibrary.org/obo/GAZ_00004381 -->

    <owl:NamedIndividual rdf:about="http://purl.obolibrary.org/obo/GAZ_00004381">
        <obo:RO_0001025 rdf:resource="http://purl.obolibrary.org/obo/GAZ_00004380"/>
        <obo:IAO_0000115>A high, mountainous island 38 mi long, which is the largest feature in the Palmer Archipelago, lying SW of Brabant Island at the SW end of the group.</obo:IAO_0000115>
        <oboInOwl:hasOBONamespace>GAZ</oboInOwl:hasOBONamespace>
        <oboInOwl:id>GAZ:00004381</oboInOwl:id>
        <rdfs:label>Anvers Island</rdfs:label>
    </owl:NamedIndividual>
    


    <!-- http://purl.obolibrary.org/obo/GAZ_00005837 -->

    <owl:NamedIndividual rdf:about="http://purl.obolibrary.org/obo/GAZ_00005837">
        <obo:RO_0001025 rdf:resource="http://purl.obolibrary.org/obo/GAZ_00014084"/>
        <obo:IAO_0000115>An isolated, mainly snow covered island, 11 mi long and 5 mi wide, located 200 mi NE of Cape Braathen, Thurston Island. The island is lofty with steep slopes, attaining a height of 1,755 m in Lars Christensen Peak. The islands is a morphologically youthful shield-like volcano. A 100-m-wide circular crater is found at the summit of the 1750 m high volcano. The island was discovered by the Russian explorer Bellingshausen in 1821, and extensive summer pack ice and its isolated location far from regular shipping lanes have restricted visits to the island. Dated samples from Peter I Island range from 0.35 to 0.1 million years old (Prestvik et al. 1990). The unmodified volcanic form of the upper part of the volcano argues that parts of it may be Holocene or even historical in age (LeMasurier and Thomson 1990).</obo:IAO_0000115>
        <oboInOwl:hasOBONamespace>GAZ</oboInOwl:hasOBONamespace>
        <oboInOwl:id>GAZ:00005837</oboInOwl:id>
        <rdfs:label>Peter I Island</rdfs:label>
    </owl:NamedIndividual>
    


    <!-- http://purl.obolibrary.org/obo/GAZ_00007288 -->

    <owl:NamedIndividual rdf:about="http://purl.obolibrary.org/obo/GAZ_00007288">
        <obo:RO_0001025 rdf:resource="http://purl.obolibrary.org/obo/GAZ_00007328"/>
        <obo:IAO_0000115>An island 11 mi long and 8 mi wide, lying between Nelson and Greenwich Islands in the South Shetland Islands.</obo:IAO_0000115>
        <oboInOwl:hasOBONamespace>GAZ</oboInOwl:hasOBONamespace>
        <oboInOwl:id>GAZ:00007288</oboInOwl:id>
        <rdfs:label>Robert Island</rdfs:label>
    </owl:NamedIndividual>
    


    <!-- http://purl.obolibrary.org/obo/GAZ_00007328 -->

    <owl:NamedIndividual rdf:about="http://purl.obolibrary.org/obo/GAZ_00007328">
        <obo:RO_0001025 rdf:resource="http://purl.obolibrary.org/obo/GAZ_00000373"/>
        <obo:IAO_0000115>A group of more than twenty islands and islets lying northward of Antarctic Peninsula and extending about 280 mi from Smith Island and Snow Island in the WSW to Elephant Island and Clarence Island in the ENE.</obo:IAO_0000115>
        <oboInOwl:hasOBONamespace>GAZ</oboInOwl:hasOBONamespace>
        <oboInOwl:id>GAZ:00007328</oboInOwl:id>
        <rdfs:label>South Shetland Islands</rdfs:label>
    </owl:NamedIndividual>
    


    <!-- http://purl.obolibrary.org/obo/GAZ_00007329 -->

    <owl:NamedIndividual rdf:about="http://purl.obolibrary.org/obo/GAZ_00007329">
        <obo:RO_0001025 rdf:resource="http://purl.obolibrary.org/obo/GAZ_00007328"/>
        <obo:IAO_0000115>An island 38 mi long and from 2 to 20 mi wide, lying between Greenwich and Snow Islands in the South Shetland Islands.</obo:IAO_0000115>
        <oboInOwl:hasOBONamespace>GAZ</oboInOwl:hasOBONamespace>
        <oboInOwl:id>GAZ:00007329</oboInOwl:id>
        <rdfs:label>Livingston Island</rdfs:label>
    </owl:NamedIndividual>
    


    <!-- http://purl.obolibrary.org/obo/GAZ_00007330 -->

    <owl:NamedIndividual rdf:about="http://purl.obolibrary.org/obo/GAZ_00007330">
        <obo:RO_0001025 rdf:resource="http://purl.obolibrary.org/obo/GAZ_00007329"/>
        <obo:IAO_0000115>Mainly ice-free peninsula forming the W end of Livingston Island, in the South Shetland Islands.</obo:IAO_0000115>
        <oboInOwl:hasOBONamespace>GAZ</oboInOwl:hasOBONamespace>
        <oboInOwl:id>GAZ:00007330</oboInOwl:id>
        <rdfs:label>Byers Peninsula</rdfs:label>
    </owl:NamedIndividual>
    


    <!-- http://purl.obolibrary.org/obo/GAZ_00007425 -->

    <owl:NamedIndividual rdf:about="http://purl.obolibrary.org/obo/GAZ_00007425">
        <obo:RO_0001025 rdf:resource="http://purl.obolibrary.org/obo/GAZ_00007328"/>
        <obo:IAO_0000115>An island 43 mi long and 16 mi wide at its broadest part, lying E of Nelson Island in the South Shetland Islands.</obo:IAO_0000115>
        <oboInOwl:hasOBONamespace>GAZ</oboInOwl:hasOBONamespace>
        <oboInOwl:id>GAZ:00007425</oboInOwl:id>
        <rdfs:label>King George Island</rdfs:label>
    </owl:NamedIndividual>
    


    <!-- http://purl.obolibrary.org/obo/GAZ_00007426 -->

    <owl:NamedIndividual rdf:about="http://purl.obolibrary.org/obo/GAZ_00007426">
        <obo:RO_0001025 rdf:resource="http://purl.obolibrary.org/obo/GAZ_00140059"/>
        <obo:IAO_0000115>An irregular bay, 5 mi wide at its entrance between Demay Point and Martins Head, indenting the S coast of King George Island for 10 mi in the South Shetland Islands.</obo:IAO_0000115>
        <oboInOwl:hasOBONamespace>GAZ</oboInOwl:hasOBONamespace>
        <oboInOwl:id>GAZ:00007426</oboInOwl:id>
        <rdfs:label>Admiralty Bay</rdfs:label>
    </owl:NamedIndividual>
    


    <!-- http://purl.obolibrary.org/obo/GAZ_00007475 -->

    <owl:NamedIndividual rdf:about="http://purl.obolibrary.org/obo/GAZ_00007475">
        <obo:RO_0001025 rdf:resource="http://purl.obolibrary.org/obo/GAZ_00139422"/>
        <obo:IAO_0000115>A deep embayment of Antarctica between the Lars Christensen Coast and Ingrid Christensen Coast.</obo:IAO_0000115>
        <oboInOwl:hasOBONamespace>GAZ</oboInOwl:hasOBONamespace>
        <oboInOwl:id>GAZ:00007475</oboInOwl:id>
        <rdfs:label>Prydz Bay</rdfs:label>
    </owl:NamedIndividual>
    


    <!-- http://purl.obolibrary.org/obo/GAZ_00007628 -->

    <owl:NamedIndividual rdf:about="http://purl.obolibrary.org/obo/GAZ_00007628">
        <obo:RO_0001025 rdf:resource="http://purl.obolibrary.org/obo/GAZ_00004057"/>
        <obo:IAO_0000115>A small elongate lake 0.5 mi N of Cape Barne, Ross Island.</obo:IAO_0000115>
        <oboInOwl:hasOBONamespace>GAZ</oboInOwl:hasOBONamespace>
        <oboInOwl:id>GAZ:00007628</oboInOwl:id>
        <rdfs:label>Deep Lake</rdfs:label>
    </owl:NamedIndividual>
    


    <!-- http://purl.obolibrary.org/obo/GAZ_00007680 -->

    <owl:NamedIndividual rdf:about="http://purl.obolibrary.org/obo/GAZ_00007680">
        <obo:RO_0001025 rdf:resource="http://purl.obolibrary.org/obo/GAZ_00009005"/>
        <obo:IAO_0000115>The northernmost lake in Three Lakes Valley in northeastern Signy Island.</obo:IAO_0000115>
        <oboInOwl:hasOBONamespace>GAZ</oboInOwl:hasOBONamespace>
        <oboInOwl:id>GAZ:00007680</oboInOwl:id>
        <rdfs:label>Heywood Lake</rdfs:label>
    </owl:NamedIndividual>
    


    <!-- http://purl.obolibrary.org/obo/GAZ_00007851 -->

    <owl:NamedIndividual rdf:about="http://purl.obolibrary.org/obo/GAZ_00007851">
        <obo:RO_0001025 rdf:resource="http://purl.obolibrary.org/obo/GAZ_00051500"/>
        <obo:IAO_0000115>An area of bare rocky hills and islands along the east shore of Lutzow-Holmbukta.</obo:IAO_0000115>
        <oboInOwl:hasOBONamespace>GAZ</oboInOwl:hasOBONamespace>
        <oboInOwl:id>GAZ:00007851</oboInOwl:id>
        <rdfs:label>Langhovde</rdfs:label>
    </owl:NamedIndividual>
    


    <!-- http://purl.obolibrary.org/obo/GAZ_00009005 -->

    <owl:NamedIndividual rdf:about="http://purl.obolibrary.org/obo/GAZ_00009005">
        <obo:RO_0001025 rdf:resource="http://purl.obolibrary.org/obo/GAZ_00009523"/>
        <obo:IAO_0000115>An island 4 mi long and less than 3 mi wide, lying close S of the middle of Coronation Island, in the South Orkney Islands.</obo:IAO_0000115>
        <oboInOwl:hasOBONamespace>GAZ</oboInOwl:hasOBONamespace>
        <oboInOwl:id>GAZ:00009005</oboInOwl:id>
        <rdfs:label>Signy Island</rdfs:label>
    </owl:NamedIndividual>
    


    <!-- http://purl.obolibrary.org/obo/GAZ_00009523 -->

    <owl:NamedIndividual rdf:about="http://purl.obolibrary.org/obo/GAZ_00009523">
        <obo:RO_0001025 rdf:resource="http://purl.obolibrary.org/obo/GAZ_00000373"/>
        <obo:IAO_0000115>A group of two larger and several smaller mountainous, barren islands covered with ice and snow and surrounded by many rocks, lying NE of the Antarctic Peninsula between 6020S and 6050S, and 4420W and 46457W.</obo:IAO_0000115>
        <oboInOwl:hasOBONamespace>GAZ</oboInOwl:hasOBONamespace>
        <oboInOwl:id>GAZ:00009523</oboInOwl:id>
        <rdfs:label>South Orkney Islands</rdfs:label>
    </owl:NamedIndividual>
    


    <!-- http://purl.obolibrary.org/obo/GAZ_00011769 -->

    <owl:NamedIndividual rdf:about="http://purl.obolibrary.org/obo/GAZ_00011769">
        <obo:RO_0001025 rdf:resource="http://purl.obolibrary.org/obo/GAZ_00023304"/>
        <oboInOwl:hasOBONamespace>GAZ</oboInOwl:hasOBONamespace>
        <oboInOwl:id>GAZ:00011769</oboInOwl:id>
        <rdfs:label>Ross Ice Shelf</rdfs:label>
    </owl:NamedIndividual>
    


    <!-- http://purl.obolibrary.org/obo/GAZ_00011782 -->

    <owl:NamedIndividual rdf:about="http://purl.obolibrary.org/obo/GAZ_00011782">
        <obo:RO_0001025 rdf:resource="http://purl.obolibrary.org/obo/GAZ_00023304"/>
        <obo:IAO_0000115>A bay which is often ice free, about 64 km long, lying between Cape Washington and the Drygalski Ice Tongue along the coast of Victoria Land, Antarctica.</obo:IAO_0000115>
        <oboInOwl:hasOBONamespace>GAZ</oboInOwl:hasOBONamespace>
        <oboInOwl:id>GAZ:00011782</oboInOwl:id>
        <rdfs:label>Terra Nova Bay</rdfs:label>
    </owl:NamedIndividual>
    


    <!-- http://purl.obolibrary.org/obo/GAZ_00014084 -->

    <owl:NamedIndividual rdf:about="http://purl.obolibrary.org/obo/GAZ_00014084">
        <obo:RO_0001025 rdf:resource="http://purl.obolibrary.org/obo/GAZ_00000373"/>
        <obo:IAO_0000115>A sea along the west side of the Antarctic Peninsula between Alexander Island and Thurston Island, approximately between 102degW and 70degW.</obo:IAO_0000115>
        <oboInOwl:hasOBONamespace>GAZ</oboInOwl:hasOBONamespace>
        <oboInOwl:id>GAZ:00014084</oboInOwl:id>
        <rdfs:label>Bellingshausen Sea</rdfs:label>
    </owl:NamedIndividual>
    


    <!-- http://purl.obolibrary.org/obo/GAZ_00014085 -->

    <owl:NamedIndividual rdf:about="http://purl.obolibrary.org/obo/GAZ_00014085">
        <rdf:type rdf:resource="http://purl.obolibrary.org/obo/ENVO_00000475"/>
        <obo:RO_0001025 rdf:resource="http://purl.obolibrary.org/obo/GAZ_00000373"/>
        <obo:IAO_0000115>An arm of the Southern Ocean off Marie Byrd Land in western Antarctica. It is bounded by Cape Flying Fish, Thurston Island, at 102deg20minW, to the east and Cape Dart, at 126deg9minW, to the west.</obo:IAO_0000115>
        <oboInOwl:hasOBONamespace>GAZ</oboInOwl:hasOBONamespace>
        <oboInOwl:id>GAZ:00014085</oboInOwl:id>
        <rdfs:label>Amundsen Sea</rdfs:label>
    </owl:NamedIndividual>
    


    <!-- http://purl.obolibrary.org/obo/GAZ_00014088 -->

    <owl:NamedIndividual rdf:about="http://purl.obolibrary.org/obo/GAZ_00014088">
        <obo:RO_0001025 rdf:resource="http://purl.obolibrary.org/obo/GAZ_00014084"/>
        <obo:IAO_0000115>The largest island of Antarctica, with an area of 43,250 km2 lying in the Bellingshausen Sea west of the base of the Antarctic Peninsula, from which it is separated by Marguerite Bay and George VI Sound. Alexander Island lies off the coast of Antarctica and is linked to it by an ice shelf.</obo:IAO_0000115>
        <oboInOwl:hasOBONamespace>GAZ</oboInOwl:hasOBONamespace>
        <oboInOwl:id>GAZ:00014088</oboInOwl:id>
        <rdfs:label>Alexander Island</rdfs:label>
    </owl:NamedIndividual>
    


    <!-- http://purl.obolibrary.org/obo/GAZ_00014089 -->

    <owl:NamedIndividual rdf:about="http://purl.obolibrary.org/obo/GAZ_00014089">
        <obo:RO_0001025 rdf:resource="http://purl.obolibrary.org/obo/GAZ_00141552"/>
        <obo:IAO_0000115>An extensive bay on the west side of the Antarctic Peninsula, which is bounded on the north by Adelaide Island and on the south by Wordie Ice Shelf, George VI Sound and Alexander Island.</obo:IAO_0000115>
        <oboInOwl:hasOBONamespace>GAZ</oboInOwl:hasOBONamespace>
        <oboInOwl:id>GAZ:00014089</oboInOwl:id>
        <rdfs:label>Marguerite Bay</rdfs:label>
    </owl:NamedIndividual>
    


    <!-- http://purl.obolibrary.org/obo/GAZ_00014090 -->

    <owl:NamedIndividual rdf:about="http://purl.obolibrary.org/obo/GAZ_00014090">
        <obo:RO_0001025 rdf:resource="http://purl.obolibrary.org/obo/GAZ_00014084"/>
        <obo:IAO_0000115>A major bay/fault depression, 483 km long in the shape of the letter J, which skirts the east and south shores of Alexander Island, separating it from the Antarctic Peninsula and the English Coast.</obo:IAO_0000115>
        <oboInOwl:hasOBONamespace>GAZ</oboInOwl:hasOBONamespace>
        <oboInOwl:id>GAZ:00014090</oboInOwl:id>
        <rdfs:label>George VI Sound</rdfs:label>
    </owl:NamedIndividual>
    


    <!-- http://purl.obolibrary.org/obo/GAZ_00014091 -->

    <owl:NamedIndividual rdf:about="http://purl.obolibrary.org/obo/GAZ_00014091">
        <obo:RO_0001025 rdf:resource="http://purl.obolibrary.org/obo/GAZ_00051517"/>
        <obo:IAO_0000115>A small island just off the west side of the Antarctic Peninsula of Antarctica, located at 65 deg 10 min S, 64 deg 10 min W, just a short distance south of Booth Island and the Lemaire Channel.</obo:IAO_0000115>
        <oboInOwl:hasOBONamespace>GAZ</oboInOwl:hasOBONamespace>
        <oboInOwl:id>GAZ:00014091</oboInOwl:id>
        <rdfs:label>Petermann Island</rdfs:label>
    </owl:NamedIndividual>
    


    <!-- http://purl.obolibrary.org/obo/GAZ_00014093 -->

    <owl:NamedIndividual rdf:about="http://purl.obolibrary.org/obo/GAZ_00014093">
        <obo:RO_0001025 rdf:resource="http://purl.obolibrary.org/obo/GAZ_00014094"/>
        <obo:IAO_0000115>A rocky Antarctic island, 1.5 mi long, between Ardery Island and Robinson Ridge in the Windmill Islands.</obo:IAO_0000115>
        <oboInOwl:hasOBONamespace>GAZ</oboInOwl:hasOBONamespace>
        <oboInOwl:id>GAZ:00014093</oboInOwl:id>
        <rdfs:label>Odbert Island</rdfs:label>
    </owl:NamedIndividual>
    


    <!-- http://purl.obolibrary.org/obo/GAZ_00014094 -->

    <owl:NamedIndividual rdf:about="http://purl.obolibrary.org/obo/GAZ_00014094">
        <obo:RO_0001025 rdf:resource="http://purl.obolibrary.org/obo/GAZ_00014108"/>
        <obo:IAO_0000115>An Antarctic group of rocky islands and rocks about 6 mi wide, paralleling the coast of Wilkes Land for 17 mi immediately north of Vanderford Glacier along the east side of Vincennes Bay.</obo:IAO_0000115>
        <oboInOwl:hasOBONamespace>GAZ</oboInOwl:hasOBONamespace>
        <oboInOwl:id>GAZ:00014094</oboInOwl:id>
        <rdfs:label>Windmill Islands</rdfs:label>
    </owl:NamedIndividual>
    


    <!-- http://purl.obolibrary.org/obo/GAZ_00014095 -->

    <owl:NamedIndividual rdf:about="http://purl.obolibrary.org/obo/GAZ_00014095">
        <obo:RO_0001025 rdf:resource="http://purl.obolibrary.org/obo/GAZ_00007328"/>
        <obo:IAO_0000115>An island on the W side of Maxwell Bay, King George Island.</obo:IAO_0000115>
        <oboInOwl:hasOBONamespace>GAZ</oboInOwl:hasOBONamespace>
        <oboInOwl:id>GAZ:00014095</oboInOwl:id>
        <rdfs:label>Ardley Island</rdfs:label>
    </owl:NamedIndividual>
    


    <!-- http://purl.obolibrary.org/obo/GAZ_00014096 -->

    <owl:NamedIndividual rdf:about="http://purl.obolibrary.org/obo/GAZ_00014096">
        <obo:RO_0001025 rdf:resource="http://purl.obolibrary.org/obo/GAZ_00023304"/>
        <obo:IAO_0000115>A convenient name for that group of islands which, together with the ice shelf between them, forms the eastern and southern boundaries of McMurdo Sound.</obo:IAO_0000115>
        <oboInOwl:hasOBONamespace>GAZ</oboInOwl:hasOBONamespace>
        <oboInOwl:id>GAZ:00014096</oboInOwl:id>
        <rdfs:label>Ross Archipelago</rdfs:label>
    </owl:NamedIndividual>
    


    <!-- http://purl.obolibrary.org/obo/GAZ_00014097 -->

    <owl:NamedIndividual rdf:about="http://purl.obolibrary.org/obo/GAZ_00014097">
        <obo:RO_0001025 rdf:resource="http://purl.obolibrary.org/obo/GAZ_00014096"/>
        <obo:IAO_0000115>An island in the Western Ross Ice Shelf.</obo:IAO_0000115>
        <oboInOwl:hasOBONamespace>GAZ</oboInOwl:hasOBONamespace>
        <oboInOwl:id>GAZ:00014097</oboInOwl:id>
        <rdfs:label>Black Island</rdfs:label>
    </owl:NamedIndividual>
    


    <!-- http://purl.obolibrary.org/obo/GAZ_00014098 -->

    <owl:NamedIndividual rdf:about="http://purl.obolibrary.org/obo/GAZ_00014098">
        <rdf:type rdf:resource="http://purl.obolibrary.org/obo/ENVO_00000222"/>
        <obo:RO_0001025 rdf:resource="http://purl.obolibrary.org/obo/GAZ_00014096"/>
        <obo:IAO_0000115>A volcanic island in the Ross Sea, the northernmost feature of the Ross Archipelago, lying 12 mi N of Cape Bird, Ross Island.</obo:IAO_0000115>
        <oboInOwl:hasOBONamespace>GAZ</oboInOwl:hasOBONamespace>
        <oboInOwl:id>GAZ:00014098</oboInOwl:id>
        <rdfs:label>Beaufort Island</rdfs:label>
    </owl:NamedIndividual>
    


    <!-- http://purl.obolibrary.org/obo/GAZ_00014099 -->

    <owl:NamedIndividual rdf:about="http://purl.obolibrary.org/obo/GAZ_00014099">
        <obo:RO_0001025 rdf:resource="http://purl.obolibrary.org/obo/GAZ_00014096"/>
        <obo:IAO_0000115>A group of four islands lying in the Antarctic, just south of Cape Evans and Ross Island.</obo:IAO_0000115>
        <oboInOwl:hasOBONamespace>GAZ</oboInOwl:hasOBONamespace>
        <oboInOwl:id>GAZ:00014099</oboInOwl:id>
        <rdfs:label>Dellbridge Islands</rdfs:label>
    </owl:NamedIndividual>
    


    <!-- http://purl.obolibrary.org/obo/GAZ_00014100 -->

    <owl:NamedIndividual rdf:about="http://purl.obolibrary.org/obo/GAZ_00014100">
        <obo:RO_0001025 rdf:resource="http://purl.obolibrary.org/obo/GAZ_00014096"/>
        <oboInOwl:hasOBONamespace>GAZ</oboInOwl:hasOBONamespace>
        <oboInOwl:id>GAZ:00014100</oboInOwl:id>
        <rdfs:label>White Island</rdfs:label>
    </owl:NamedIndividual>
    


    <!-- http://purl.obolibrary.org/obo/GAZ_00014102 -->

    <owl:NamedIndividual rdf:about="http://purl.obolibrary.org/obo/GAZ_00014102">
        <obo:RO_0001025 rdf:resource="http://purl.obolibrary.org/obo/GAZ_00007425"/>
        <oboInOwl:hasOBONamespace>GAZ</oboInOwl:hasOBONamespace>
        <oboInOwl:id>GAZ:00014102</oboInOwl:id>
        <rdfs:label>Botany Point</rdfs:label>
    </owl:NamedIndividual>
    


    <!-- http://purl.obolibrary.org/obo/GAZ_00014104 -->

    <owl:NamedIndividual rdf:about="http://purl.obolibrary.org/obo/GAZ_00014104">
        <obo:RO_0001025 rdf:resource="http://purl.obolibrary.org/obo/GAZ_00004057"/>
        <obo:IAO_0000115>An ice-covered cape forming the E end of Ross Island.</obo:IAO_0000115>
        <oboInOwl:hasOBONamespace>GAZ</oboInOwl:hasOBONamespace>
        <oboInOwl:id>GAZ:00014104</oboInOwl:id>
        <rdfs:label>Cape Crozier</rdfs:label>
    </owl:NamedIndividual>
    


    <!-- http://purl.obolibrary.org/obo/GAZ_00014105 -->

    <owl:NamedIndividual rdf:about="http://purl.obolibrary.org/obo/GAZ_00014105">
        <obo:RO_0001025 rdf:resource="http://purl.obolibrary.org/obo/GAZ_00004057"/>
        <obo:IAO_0000115>A dark rock cape forming the west extremity of Ross Island, facing on McMurdo Sound.</obo:IAO_0000115>
        <oboInOwl:hasOBONamespace>GAZ</oboInOwl:hasOBONamespace>
        <oboInOwl:id>GAZ:00014105</oboInOwl:id>
        <rdfs:label>Cape Royds</rdfs:label>
    </owl:NamedIndividual>
    


    <!-- http://purl.obolibrary.org/obo/GAZ_00014106 -->

    <owl:NamedIndividual rdf:about="http://purl.obolibrary.org/obo/GAZ_00014106">
        <obo:RO_0001025 rdf:resource="http://purl.obolibrary.org/obo/GAZ_00014108"/>
        <obo:IAO_0000115>A permanent base in Antarctica managed by the Australian Antarctic Division (AAD) located on Vincennes Bay.</obo:IAO_0000115>
        <oboInOwl:hasOBONamespace>GAZ</oboInOwl:hasOBONamespace>
        <oboInOwl:id>GAZ:00014106</oboInOwl:id>
        <rdfs:label>Casey Station</rdfs:label>
    </owl:NamedIndividual>
    


    <!-- http://purl.obolibrary.org/obo/GAZ_00014108 -->

    <owl:NamedIndividual rdf:about="http://purl.obolibrary.org/obo/GAZ_00014108">
        <obo:RO_0001025 rdf:resource="http://purl.obolibrary.org/obo/GAZ_00141023"/>
        <obo:IAO_0000115>A large V-shaped bay, 105 km wide at its entrance between Cape Nutt and Cape Folger and marked by several large, steep glaciers near its head, lying along Knox and Budd Coasts.</obo:IAO_0000115>
        <oboInOwl:hasOBONamespace>GAZ</oboInOwl:hasOBONamespace>
        <oboInOwl:id>GAZ:00014108</oboInOwl:id>
        <rdfs:label>Vincennes Bay</rdfs:label>
    </owl:NamedIndividual>
    


    <!-- http://purl.obolibrary.org/obo/GAZ_00014109 -->

    <owl:NamedIndividual rdf:about="http://purl.obolibrary.org/obo/GAZ_00014109">
        <obo:RO_0001025 rdf:resource="http://purl.obolibrary.org/obo/GAZ_00014110"/>
        <obo:IAO_0000115>The main Argentine base in Antarctica, and it is located in Seymour Island.</obo:IAO_0000115>
        <oboInOwl:hasOBONamespace>GAZ</oboInOwl:hasOBONamespace>
        <oboInOwl:id>GAZ:00014109</oboInOwl:id>
        <rdfs:label>Marambio Base</rdfs:label>
    </owl:NamedIndividual>
    


    <!-- http://purl.obolibrary.org/obo/GAZ_00014110 -->

    <owl:NamedIndividual rdf:about="http://purl.obolibrary.org/obo/GAZ_00014110">
        <obo:RO_0001025 rdf:resource="http://purl.obolibrary.org/obo/GAZ_00004045"/>
        <obo:IAO_0000115>An island in the chain of 16 major islands around the tip of the Graham Land on the Antarctic Peninsula. Within the island chain, it is located west of the peninsula, off the north tip of Snow Hill Island and just of east of the larger key, James Ross Island, and it&apos;s smaller neighboring island, Vega Island.</obo:IAO_0000115>
        <oboInOwl:hasOBONamespace>GAZ</oboInOwl:hasOBONamespace>
        <oboInOwl:id>GAZ:00014110</oboInOwl:id>
        <rdfs:label>Seymour Island</rdfs:label>
    </owl:NamedIndividual>
    


    <!-- http://purl.obolibrary.org/obo/GAZ_00014111 -->

    <owl:NamedIndividual rdf:about="http://purl.obolibrary.org/obo/GAZ_00014111">
        <obo:RO_0001025 rdf:resource="http://purl.obolibrary.org/obo/GAZ_00004381"/>
        <obo:IAO_0000115>A United States research station. Established in 1968.</obo:IAO_0000115>
        <oboInOwl:hasOBONamespace>GAZ</oboInOwl:hasOBONamespace>
        <oboInOwl:id>GAZ:00014111</oboInOwl:id>
        <rdfs:label>Palmer Station</rdfs:label>
    </owl:NamedIndividual>
    


    <!-- http://purl.obolibrary.org/obo/GAZ_00014112 -->

    <owl:NamedIndividual rdf:about="http://purl.obolibrary.org/obo/GAZ_00014112">
        <obo:RO_0001025 rdf:resource="http://purl.obolibrary.org/obo/GAZ_00023358"/>
        <obo:IAO_0000115>A research station, now New Zealand operated, on Ross Island.</obo:IAO_0000115>
        <oboInOwl:hasOBONamespace>GAZ</oboInOwl:hasOBONamespace>
        <oboInOwl:id>GAZ:00014112</oboInOwl:id>
        <rdfs:label>Scott Base</rdfs:label>
    </owl:NamedIndividual>
    


    <!-- http://purl.obolibrary.org/obo/GAZ_00014113 -->

    <owl:NamedIndividual rdf:about="http://purl.obolibrary.org/obo/GAZ_00014113">
        <obo:RO_0001025 rdf:resource="http://purl.obolibrary.org/obo/GAZ_00007328"/>
        <obo:IAO_0000115>An ice-covered, mountainous island off the coast of Antarctica in the outer reaches of the South Shetland Islands in the Southern Ocean.</obo:IAO_0000115>
        <oboInOwl:hasOBONamespace>GAZ</oboInOwl:hasOBONamespace>
        <oboInOwl:id>GAZ:00014113</oboInOwl:id>
        <rdfs:label>Elephant Island</rdfs:label>
    </owl:NamedIndividual>
    


    <!-- http://purl.obolibrary.org/obo/GAZ_00014114 -->

    <owl:NamedIndividual rdf:about="http://purl.obolibrary.org/obo/GAZ_00014114">
        <obo:RO_0001025 rdf:resource="http://purl.obolibrary.org/obo/GAZ_00011782"/>
        <obo:IAO_0000115>A rocky island located in Terra Nova Bay.</obo:IAO_0000115>
        <oboInOwl:hasOBONamespace>GAZ</oboInOwl:hasOBONamespace>
        <oboInOwl:id>GAZ:00014114</oboInOwl:id>
        <rdfs:label>Inexpressible Island</rdfs:label>
    </owl:NamedIndividual>
    


    <!-- http://purl.obolibrary.org/obo/GAZ_00014115 -->

    <owl:NamedIndividual rdf:about="http://purl.obolibrary.org/obo/GAZ_00014115">
        <obo:RO_0001025 rdf:resource="http://purl.obolibrary.org/obo/GAZ_00051134"/>
        <obo:IAO_0000115>A South Korean research station. Established 1988-02-17.</obo:IAO_0000115>
        <oboInOwl:hasOBONamespace>GAZ</oboInOwl:hasOBONamespace>
        <oboInOwl:id>GAZ:00014115</oboInOwl:id>
        <rdfs:label>King Sejong Station</rdfs:label>
    </owl:NamedIndividual>
    


    <!-- http://purl.obolibrary.org/obo/GAZ_00014119 -->

    <owl:NamedIndividual rdf:about="http://purl.obolibrary.org/obo/GAZ_00014119">
        <obo:RO_0001025 rdf:resource="http://purl.obolibrary.org/obo/GAZ_00004057"/>
        <obo:IAO_0000115>A stratovolcano that overlooks the McMurdo research station on Ross Island. The 3794 m high Erebus is the largest of three major volcanoes forming the crudely triangular Ross Island. The summit of the dominantly phonolitic Mount Erebus has been modified by one or two generations of caldera formation. A summit plateau at about 3200-m altitude marks the rim of the youngest caldera, which formed during the late-Pleistocene and within which the modern cone was constructed. An elliptical 500 x 600 m wide, 110-m-deep crater truncates the summit and contains an active lava lake within a 250-m-wide, 100-m-deep inner crater. The glacier-covered volcano was erupting when first sighted by Captain James Ross in 1841. Continuous lava-lake activity with minor explosions, punctuated by occasional larger strombolian explosions that eject bombs onto the crater rim, has been documented since 1972, but has probably been occurring for much of the volcano&apos;s recent history.</obo:IAO_0000115>
        <oboInOwl:hasOBONamespace>GAZ</oboInOwl:hasOBONamespace>
        <oboInOwl:id>GAZ:00014119</oboInOwl:id>
        <rdfs:label>Mount Erebus</rdfs:label>
    </owl:NamedIndividual>
    


    <!-- http://purl.obolibrary.org/obo/GAZ_00014120 -->

    <owl:NamedIndividual rdf:about="http://purl.obolibrary.org/obo/GAZ_00014120">
        <obo:RO_0001025 rdf:resource="http://purl.obolibrary.org/obo/GAZ_00007328"/>
        <obo:IAO_0000115>An island 19 km long and 11 km wide, lying southwest of King George Island in the South Shetland Islands.</obo:IAO_0000115>
        <oboInOwl:hasOBONamespace>GAZ</oboInOwl:hasOBONamespace>
        <oboInOwl:id>GAZ:00014120</oboInOwl:id>
        <rdfs:label>Nelson Island</rdfs:label>
    </owl:NamedIndividual>
    


    <!-- http://purl.obolibrary.org/obo/GAZ_00014121 -->

    <owl:NamedIndividual rdf:about="http://purl.obolibrary.org/obo/GAZ_00014121">
        <obo:RO_0001025 rdf:resource="http://purl.obolibrary.org/obo/GAZ_00007328"/>
        <obo:IAO_0000115>An island in the South Shetland Islands off the Antarctic Peninsula which has one of the safest harbours in Antarctica. A recently active volcano, its eruptions in 1967 and 1969 caused serious damage to the scientific stations there.</obo:IAO_0000115>
        <oboInOwl:hasOBONamespace>GAZ</oboInOwl:hasOBONamespace>
        <oboInOwl:id>GAZ:00014121</oboInOwl:id>
        <rdfs:label>Deception Island</rdfs:label>
    </owl:NamedIndividual>
    


    <!-- http://purl.obolibrary.org/obo/GAZ_00014122 -->

    <owl:NamedIndividual rdf:about="http://purl.obolibrary.org/obo/GAZ_00014122">
        <obo:RO_0001025 rdf:resource="http://purl.obolibrary.org/obo/GAZ_00141552"/>
        <obo:IAO_0000115>An island archipelago off the west coast of the Antarctic Peninsula in Antarctica. Consists of a myriad of islands, the largest of which are Booth Island and Hovgaard Island. The archipelago extends from Bismarck Strait southwest to Lumus Rock, off the west coast of Graham Land.</obo:IAO_0000115>
        <oboInOwl:hasOBONamespace>GAZ</oboInOwl:hasOBONamespace>
        <oboInOwl:id>GAZ:00014122</oboInOwl:id>
        <rdfs:label>Wilhelm Archipelago</rdfs:label>
    </owl:NamedIndividual>
    


    <!-- http://purl.obolibrary.org/obo/GAZ_00014123 -->

    <owl:NamedIndividual rdf:about="http://purl.obolibrary.org/obo/GAZ_00014123">
        <obo:RO_0001025 rdf:resource="http://purl.obolibrary.org/obo/GAZ_00051518"/>
        <oboInOwl:hasOBONamespace>GAZ</oboInOwl:hasOBONamespace>
        <oboInOwl:id>GAZ:00014123</oboInOwl:id>
        <rdfs:label>Galindez Island</rdfs:label>
    </owl:NamedIndividual>
    


    <!-- http://purl.obolibrary.org/obo/GAZ_00014124 -->

    <owl:NamedIndividual rdf:about="http://purl.obolibrary.org/obo/GAZ_00014124">
        <obo:RO_0001025 rdf:resource="http://purl.obolibrary.org/obo/GAZ_00014084"/>
        <obo:IAO_0000115>An island off Antarctica, 30 miles long and 25 miles wide, which is ice covered except for prominent mountains overlooking the north coast, 55 miles west of Alexander Island.</obo:IAO_0000115>
        <oboInOwl:hasOBONamespace>GAZ</oboInOwl:hasOBONamespace>
        <oboInOwl:id>GAZ:00014124</oboInOwl:id>
        <rdfs:label>Charcot Island</rdfs:label>
    </owl:NamedIndividual>
    


    <!-- http://purl.obolibrary.org/obo/GAZ_00014125 -->

    <owl:NamedIndividual rdf:about="http://purl.obolibrary.org/obo/GAZ_00014125">
        <obo:RO_0001025 rdf:resource="http://purl.obolibrary.org/obo/GAZ_00004045"/>
    </owl:NamedIndividual>
    


    <!-- http://purl.obolibrary.org/obo/GAZ_00014140 -->

    <owl:NamedIndividual rdf:about="http://purl.obolibrary.org/obo/GAZ_00014140">
        <obo:RO_0001025 rdf:resource="http://purl.obolibrary.org/obo/GAZ_00014085"/>
        <obo:RO_0001025 rdf:resource="http://purl.obolibrary.org/obo/GAZ_00051504"/>
        <obo:IAO_0000115>An ice-covered, glacially dissected island, 215 km long, 90 km wide and 15,700 km2 in area, lying a short way off the NW end of Ellsworth Land, Antarctica. It is the third largest island of Antarctica, after Alexander Island and Berkner Island.</obo:IAO_0000115>
        <oboInOwl:hasOBONamespace>GAZ</oboInOwl:hasOBONamespace>
        <oboInOwl:id>GAZ:00014140</oboInOwl:id>
        <rdfs:label>Thurston Island</rdfs:label>
    </owl:NamedIndividual>
    


    <!-- http://purl.obolibrary.org/obo/GAZ_00017726 -->

    <owl:NamedIndividual rdf:about="http://purl.obolibrary.org/obo/GAZ_00017726">
        <obo:RO_0001025 rdf:resource="http://purl.obolibrary.org/obo/GAZ_00007328"/>
        <obo:IAO_0000115>An island 18 km long and the easternmost of the South Shetland Islands of the British Antarctic Territory.</obo:IAO_0000115>
        <oboInOwl:hasOBONamespace>GAZ</oboInOwl:hasOBONamespace>
        <oboInOwl:id>GAZ:00017726</oboInOwl:id>
        <rdfs:label>Clarence Island</rdfs:label>
    </owl:NamedIndividual>
    


    <!-- http://purl.obolibrary.org/obo/GAZ_00017727 -->

    <owl:NamedIndividual rdf:about="http://purl.obolibrary.org/obo/GAZ_00017727">
        <obo:RO_0001025 rdf:resource="http://purl.obolibrary.org/obo/GAZ_00007328"/>
        <obo:IAO_0000115>An island 20 km southwest of Elephant Island in the South Shetland Islands.</obo:IAO_0000115>
        <oboInOwl:hasOBONamespace>GAZ</oboInOwl:hasOBONamespace>
        <oboInOwl:id>GAZ:00017727</oboInOwl:id>
        <rdfs:label>Gibbs Island</rdfs:label>
    </owl:NamedIndividual>
    


    <!-- http://purl.obolibrary.org/obo/GAZ_00017728 -->

    <owl:NamedIndividual rdf:about="http://purl.obolibrary.org/obo/GAZ_00017728">
        <obo:RO_0001025 rdf:resource="http://purl.obolibrary.org/obo/GAZ_00007328"/>
        <obo:IAO_0000115>An island 1 mile long, which lies 5 miles northeast of the east end of Elephant Island, in the South Shetland Islands.</obo:IAO_0000115>
        <oboInOwl:hasOBONamespace>GAZ</oboInOwl:hasOBONamespace>
        <oboInOwl:id>GAZ:00017728</oboInOwl:id>
        <rdfs:label>Cornwallis Island</rdfs:label>
    </owl:NamedIndividual>
    


    <!-- http://purl.obolibrary.org/obo/GAZ_00017729 -->

    <owl:NamedIndividual rdf:about="http://purl.obolibrary.org/obo/GAZ_00017729">
        <obo:RO_0001025 rdf:resource="http://purl.obolibrary.org/obo/GAZ_00007328"/>
        <obo:IAO_0000115>A rocky island 0.8 km long, lying immediately off Cape Lookout, Elephant Island, in the South Shetland Islands.</obo:IAO_0000115>
        <oboInOwl:hasOBONamespace>GAZ</oboInOwl:hasOBONamespace>
        <oboInOwl:id>GAZ:00017729</oboInOwl:id>
        <rdfs:label>Rowett Island</rdfs:label>
    </owl:NamedIndividual>
    


    <!-- http://purl.obolibrary.org/obo/GAZ_00017730 -->

    <owl:NamedIndividual rdf:about="http://purl.obolibrary.org/obo/GAZ_00017730">
        <obo:RO_0001025 rdf:resource="http://purl.obolibrary.org/obo/GAZ_00007328"/>
        <obo:IAO_0000115>An almost circular, volcanic island marked by steep sides, 0.8 km long and 240 m high, lying 37 km east of King George Island (South Shetland Islands). It was constructed along the axis of the Bransfield Rift spreading center between the Shetland and Wedell tectonic plates. Bridgeman Island is located east of King George Island at the NE end of the Shetland Islands, north of the tip of Graham Land Peninsula. The 240 m high island has a gently sloping top consisting of truncated lava flows. Steep cliffs surrounding the island expose older lavas and bedded pyroclastic rocks. The extensively eroded volcano does not display youthful volcanic features. Several reports of 19th-century fumarolic activity (Catalog of Active Volcanoes of the World) may instead refer to the much younger Penguin Island (Gonzalez-Ferran, 1972).</obo:IAO_0000115>
        <oboInOwl:hasOBONamespace>GAZ</oboInOwl:hasOBONamespace>
        <oboInOwl:id>GAZ:00017730</oboInOwl:id>
        <rdfs:label>Bridgeman Island</rdfs:label>
    </owl:NamedIndividual>
    


    <!-- http://purl.obolibrary.org/obo/GAZ_00017731 -->

    <owl:NamedIndividual rdf:about="http://purl.obolibrary.org/obo/GAZ_00017731">
        <obo:RO_0001025 rdf:resource="http://purl.obolibrary.org/obo/GAZ_00007328"/>
        <obo:IAO_0000115>An island, 1.4 wide by 1.7 km long, which lies close off the south coast of King George Island and marks the eastern side of the entrance to King George Bay in the South Shetland Islands.</obo:IAO_0000115>
        <oboInOwl:hasOBONamespace>GAZ</oboInOwl:hasOBONamespace>
        <oboInOwl:id>GAZ:00017731</oboInOwl:id>
        <rdfs:label>Penguin Island</rdfs:label>
    </owl:NamedIndividual>
    


    <!-- http://purl.obolibrary.org/obo/GAZ_00017732 -->

    <owl:NamedIndividual rdf:about="http://purl.obolibrary.org/obo/GAZ_00017732">
        <obo:RO_0001025 rdf:resource="http://purl.obolibrary.org/obo/GAZ_00007328"/>
        <obo:IAO_0000115>An island 3 miles long and 1 mile wide, lying west of Livingston Island in the South Shetland Islands.</obo:IAO_0000115>
        <oboInOwl:hasOBONamespace>GAZ</oboInOwl:hasOBONamespace>
        <oboInOwl:id>GAZ:00017732</oboInOwl:id>
        <rdfs:label>Rugged Island</rdfs:label>
    </owl:NamedIndividual>
    


    <!-- http://purl.obolibrary.org/obo/GAZ_00017733 -->

    <owl:NamedIndividual rdf:about="http://purl.obolibrary.org/obo/GAZ_00017733">
        <obo:RO_0001025 rdf:resource="http://purl.obolibrary.org/obo/GAZ_00007328"/>
        <obo:IAO_0000115>A group of minor islands in the north entrance to English Strait separating Greenwich Island and Robert Island in the South Shetland Islands, Antarctica, which are situated between Dee Island to the south and Table Island to the north.</obo:IAO_0000115>
        <oboInOwl:hasOBONamespace>GAZ</oboInOwl:hasOBONamespace>
        <oboInOwl:id>GAZ:00017733</oboInOwl:id>
        <rdfs:label>Aitcho Islands</rdfs:label>
    </owl:NamedIndividual>
    


    <!-- http://purl.obolibrary.org/obo/GAZ_00017734 -->

    <owl:NamedIndividual rdf:about="http://purl.obolibrary.org/obo/GAZ_00017734">
        <obo:RO_0001025 rdf:resource="http://purl.obolibrary.org/obo/GAZ_00007328"/>
        <obo:IAO_0000115>A completely ice-covered island, 16 by 8 km in size, lying 6 km southwest of Livingston Island in the South Shetland Islands.</obo:IAO_0000115>
        <oboInOwl:hasOBONamespace>GAZ</oboInOwl:hasOBONamespace>
        <oboInOwl:id>GAZ:00017734</oboInOwl:id>
        <rdfs:label>Snow Island</rdfs:label>
    </owl:NamedIndividual>
    


    <!-- http://purl.obolibrary.org/obo/GAZ_00017735 -->

    <owl:NamedIndividual rdf:about="http://purl.obolibrary.org/obo/GAZ_00017735">
        <obo:RO_0001025 rdf:resource="http://purl.obolibrary.org/obo/GAZ_00007328"/>
        <obo:IAO_0000115>An island 24 km long and from 0.8 to 10 km wide, lying between Robert Island and Livingston Island in the South Shetland Islands.</obo:IAO_0000115>
        <oboInOwl:hasOBONamespace>GAZ</oboInOwl:hasOBONamespace>
        <oboInOwl:id>GAZ:00017735</oboInOwl:id>
        <rdfs:label>Greenwich Island</rdfs:label>
    </owl:NamedIndividual>
    


    <!-- http://purl.obolibrary.org/obo/GAZ_00017736 -->

    <owl:NamedIndividual rdf:about="http://purl.obolibrary.org/obo/GAZ_00017736">
        <obo:RO_0001025 rdf:resource="http://purl.obolibrary.org/obo/GAZ_00007328"/>
        <obo:IAO_0000115>A minor subantarctic island, lying about 120 km north of the Antarctic Peninsula.</obo:IAO_0000115>
        <oboInOwl:hasOBONamespace>GAZ</oboInOwl:hasOBONamespace>
        <oboInOwl:id>GAZ:00017736</oboInOwl:id>
        <rdfs:label>Half Moon Island</rdfs:label>
    </owl:NamedIndividual>
    


    <!-- http://purl.obolibrary.org/obo/GAZ_00017737 -->

    <owl:NamedIndividual rdf:about="http://purl.obolibrary.org/obo/GAZ_00017737">
        <obo:RO_0001025 rdf:resource="http://purl.obolibrary.org/obo/GAZ_00017733"/>
        <obo:IAO_0000115>One of the Aitcho Islands.</obo:IAO_0000115>
        <oboInOwl:hasOBONamespace>GAZ</oboInOwl:hasOBONamespace>
        <oboInOwl:id>GAZ:00017737</oboInOwl:id>
        <rdfs:label>Cecilia Island</rdfs:label>
    </owl:NamedIndividual>
    


    <!-- http://purl.obolibrary.org/obo/GAZ_00017738 -->

    <owl:NamedIndividual rdf:about="http://purl.obolibrary.org/obo/GAZ_00017738">
        <obo:RO_0001025 rdf:resource="http://purl.obolibrary.org/obo/GAZ_00017733"/>
        <obo:IAO_0000115>One of the Aitcho Islands.</obo:IAO_0000115>
        <oboInOwl:hasOBONamespace>GAZ</oboInOwl:hasOBONamespace>
        <oboInOwl:id>GAZ:00017738</oboInOwl:id>
        <rdfs:label>Emeline Island</rdfs:label>
    </owl:NamedIndividual>
    


    <!-- http://purl.obolibrary.org/obo/GAZ_00017739 -->

    <owl:NamedIndividual rdf:about="http://purl.obolibrary.org/obo/GAZ_00017739">
        <obo:RO_0001025 rdf:resource="http://purl.obolibrary.org/obo/GAZ_00017733"/>
        <obo:IAO_0000115>One of the Aitcho Islands.</obo:IAO_0000115>
        <oboInOwl:hasOBONamespace>GAZ</oboInOwl:hasOBONamespace>
        <oboInOwl:id>GAZ:00017739</oboInOwl:id>
        <rdfs:label>Morris Rock</rdfs:label>
    </owl:NamedIndividual>
    


    <!-- http://purl.obolibrary.org/obo/GAZ_00017740 -->

    <owl:NamedIndividual rdf:about="http://purl.obolibrary.org/obo/GAZ_00017740">
        <obo:RO_0001025 rdf:resource="http://purl.obolibrary.org/obo/GAZ_00017733"/>
        <obo:IAO_0000115>One of the Aitcho Islands.</obo:IAO_0000115>
        <oboInOwl:hasOBONamespace>GAZ</oboInOwl:hasOBONamespace>
        <oboInOwl:id>GAZ:00017740</oboInOwl:id>
        <rdfs:label>Passage Rock</rdfs:label>
    </owl:NamedIndividual>
    


    <!-- http://purl.obolibrary.org/obo/GAZ_00017741 -->

    <owl:NamedIndividual rdf:about="http://purl.obolibrary.org/obo/GAZ_00017741">
        <obo:RO_0001025 rdf:resource="http://purl.obolibrary.org/obo/GAZ_00017733"/>
        <obo:IAO_0000115>One of the Aitcho Islands.</obo:IAO_0000115>
        <oboInOwl:hasOBONamespace>GAZ</oboInOwl:hasOBONamespace>
        <oboInOwl:id>GAZ:00017741</oboInOwl:id>
        <rdfs:label>Jorge Island</rdfs:label>
    </owl:NamedIndividual>
    


    <!-- http://purl.obolibrary.org/obo/GAZ_00017742 -->

    <owl:NamedIndividual rdf:about="http://purl.obolibrary.org/obo/GAZ_00017742">
        <obo:RO_0001025 rdf:resource="http://purl.obolibrary.org/obo/GAZ_00017733"/>
        <obo:IAO_0000115>One of the Aitcho Islands.</obo:IAO_0000115>
        <oboInOwl:hasOBONamespace>GAZ</oboInOwl:hasOBONamespace>
        <oboInOwl:id>GAZ:00017742</oboInOwl:id>
        <rdfs:label>Barrientos Island</rdfs:label>
    </owl:NamedIndividual>
    


    <!-- http://purl.obolibrary.org/obo/GAZ_00017743 -->

    <owl:NamedIndividual rdf:about="http://purl.obolibrary.org/obo/GAZ_00017743">
        <obo:RO_0001025 rdf:resource="http://purl.obolibrary.org/obo/GAZ_00017733"/>
        <obo:IAO_0000115>A narrow island which is marked by a series of small elevations throughout its length, lying 0.8 km northwest of Dee Island in the South Shetland Islands.</obo:IAO_0000115>
        <oboInOwl:hasOBONamespace>GAZ</oboInOwl:hasOBONamespace>
        <oboInOwl:id>GAZ:00017743</oboInOwl:id>
        <rdfs:label>Sierra Island</rdfs:label>
    </owl:NamedIndividual>
    


    <!-- http://purl.obolibrary.org/obo/GAZ_00017744 -->

    <owl:NamedIndividual rdf:about="http://purl.obolibrary.org/obo/GAZ_00017744">
        <obo:RO_0001025 rdf:resource="http://purl.obolibrary.org/obo/GAZ_00007328"/>
        <obo:IAO_0000115>An island 9 miles long and 5 miles wide, lying 14 miles southeast of Smith Island, in the South Shetland Islands.</obo:IAO_0000115>
        <oboInOwl:hasOBONamespace>GAZ</oboInOwl:hasOBONamespace>
        <oboInOwl:id>GAZ:00017744</oboInOwl:id>
        <rdfs:label>Low Island</rdfs:label>
    </owl:NamedIndividual>
    


    <!-- http://purl.obolibrary.org/obo/GAZ_00017745 -->

    <owl:NamedIndividual rdf:about="http://purl.obolibrary.org/obo/GAZ_00017745">
        <obo:RO_0001025 rdf:resource="http://purl.obolibrary.org/obo/GAZ_00007328"/>
        <obo:IAO_0000115>An island 32 km long and 8 km wide, lying 72 km west of Deception Island in the South Shetland Islands of the British Antarctic Territory.</obo:IAO_0000115>
        <oboInOwl:hasOBONamespace>GAZ</oboInOwl:hasOBONamespace>
        <oboInOwl:id>GAZ:00017745</oboInOwl:id>
        <rdfs:label>Smith Island</rdfs:label>
    </owl:NamedIndividual>
    


    <!-- http://purl.obolibrary.org/obo/GAZ_00017746 -->

    <owl:NamedIndividual rdf:about="http://purl.obolibrary.org/obo/GAZ_00017746">
        <obo:RO_0001025 rdf:resource="http://purl.obolibrary.org/obo/GAZ_00007328"/>
        <obo:IAO_0000115>A group of small islands and rocks lying from 3 to 6 miles northwest of Elephant Island in the South Shetland Islands.</obo:IAO_0000115>
        <oboInOwl:hasOBONamespace>GAZ</oboInOwl:hasOBONamespace>
        <oboInOwl:id>GAZ:00017746</oboInOwl:id>
        <rdfs:label>Seal Islands</rdfs:label>
    </owl:NamedIndividual>
    


    <!-- http://purl.obolibrary.org/obo/GAZ_00023248 -->

    <owl:NamedIndividual rdf:about="http://purl.obolibrary.org/obo/GAZ_00023248">
        <obo:RO_0001025 rdf:resource="http://purl.obolibrary.org/obo/GAZ_00004045"/>
        <obo:IAO_0000115>The northernmost of the Leonie Islands, lying in the entrance to Ryder Bay on the SE side of Adelaide Island.</obo:IAO_0000115>
        <oboInOwl:hasOBONamespace>GAZ</oboInOwl:hasOBONamespace>
        <oboInOwl:id>GAZ:00023248</oboInOwl:id>
        <rdfs:label>Lagoon Island</rdfs:label>
    </owl:NamedIndividual>
    


    <!-- http://purl.obolibrary.org/obo/GAZ_00023276 -->

    <owl:NamedIndividual rdf:about="http://purl.obolibrary.org/obo/GAZ_00023276">
        <rdf:type rdf:resource="http://purl.obolibrary.org/obo/ENVO_00000032"/>
        <obo:RO_0001025 rdf:resource="http://purl.obolibrary.org/obo/GAZ_00051499"/>
        <obo:IAO_0000115>An embayment on the coast of George V Land, between Cape Denison and Cape Hunter.</obo:IAO_0000115>
        <oboInOwl:hasOBONamespace>GAZ</oboInOwl:hasOBONamespace>
        <oboInOwl:id>GAZ:00023276</oboInOwl:id>
        <rdfs:label>Commonwealth Bay</rdfs:label>
    </owl:NamedIndividual>
    


    <!-- http://purl.obolibrary.org/obo/GAZ_00023278 -->

    <owl:NamedIndividual rdf:about="http://purl.obolibrary.org/obo/GAZ_00023278">
        <obo:RO_0001025 rdf:resource="http://purl.obolibrary.org/obo/GAZ_00141554"/>
        <obo:IAO_0000115>A coastal sea extending between Trollunga and Sedovodden and bordering Princesse Astrid Kyst.</obo:IAO_0000115>
        <oboInOwl:hasOBONamespace>GAZ</oboInOwl:hasOBONamespace>
        <oboInOwl:id>GAZ:00023278</oboInOwl:id>
        <rdfs:label>Lazarev Sea</rdfs:label>
    </owl:NamedIndividual>
    


    <!-- http://purl.obolibrary.org/obo/GAZ_00023280 -->

    <owl:NamedIndividual rdf:about="http://purl.obolibrary.org/obo/GAZ_00023280">
        <obo:RO_0001025 rdf:resource="http://purl.obolibrary.org/obo/GAZ_00023304"/>
        <obo:IAO_0000115>A bay in the coast of Victoria Land, about 14 mi long, entered between Cape Archer and Cape Roberts.</obo:IAO_0000115>
        <oboInOwl:hasOBONamespace>GAZ</oboInOwl:hasOBONamespace>
        <oboInOwl:id>GAZ:00023280</oboInOwl:id>
        <rdfs:label>Granite Harbour</rdfs:label>
    </owl:NamedIndividual>
    


    <!-- http://purl.obolibrary.org/obo/GAZ_00023292 -->

    <owl:NamedIndividual rdf:about="http://purl.obolibrary.org/obo/GAZ_00023292">
        <obo:RO_0001025 rdf:resource="http://purl.obolibrary.org/obo/GAZ_00011782"/>
        <obo:IAO_0000115>A research station built (in the Austral summer 1986-87) on a peninsula with NS direction along the coast of the Northern Foothills south of Gerlache Inlet (Northern Victoria Land, between Campbell Glacier and Drygalski Glacier Tongue. Named in association with the feature Terra Nova Bay into which the Station is located.</obo:IAO_0000115>
        <oboInOwl:hasOBONamespace>GAZ</oboInOwl:hasOBONamespace>
        <oboInOwl:id>GAZ:00023292</oboInOwl:id>
        <rdfs:label>Stazione Baia Terra Nova</rdfs:label>
    </owl:NamedIndividual>
    


    <!-- http://purl.obolibrary.org/obo/GAZ_00023294 -->

    <owl:NamedIndividual rdf:about="http://purl.obolibrary.org/obo/GAZ_00023294">
        <obo:RO_0001025 rdf:resource="http://purl.obolibrary.org/obo/GAZ_00051500"/>
        <obo:IAO_0000115>A large bay, about 120 mi wide, indenting the coast of Queen Maud Land between Riiser-Larsen Peninsula and the coastal angle immediately east of the Flatvaer Islands.</obo:IAO_0000115>
        <oboInOwl:hasOBONamespace>GAZ</oboInOwl:hasOBONamespace>
        <oboInOwl:id>GAZ:00023294</oboInOwl:id>
        <rdfs:label>Lutzow-Holm Bay</rdfs:label>
    </owl:NamedIndividual>
    


    <!-- http://purl.obolibrary.org/obo/GAZ_00023297 -->

    <owl:NamedIndividual rdf:about="http://purl.obolibrary.org/obo/GAZ_00023297">
        <obo:RO_0001025 rdf:resource="http://purl.obolibrary.org/obo/GAZ_00009005"/>
        <obo:IAO_0000115>The northernmost lake in Paternoster Valley in northern Signy Island.</obo:IAO_0000115>
        <oboInOwl:hasOBONamespace>GAZ</oboInOwl:hasOBONamespace>
        <oboInOwl:id>GAZ:00023297</oboInOwl:id>
        <rdfs:label>Sombre Lake</rdfs:label>
    </owl:NamedIndividual>
    


    <!-- http://purl.obolibrary.org/obo/GAZ_00023298 -->

    <owl:NamedIndividual rdf:about="http://purl.obolibrary.org/obo/GAZ_00023298">
        <obo:RO_0001025 rdf:resource="http://purl.obolibrary.org/obo/GAZ_00009005"/>
        <obo:IAO_0000115>The southernmost lake in Paternoster Valley on Signy Island.</obo:IAO_0000115>
        <oboInOwl:hasOBONamespace>GAZ</oboInOwl:hasOBONamespace>
        <oboInOwl:id>GAZ:00023298</oboInOwl:id>
        <rdfs:label>Moss Lake</rdfs:label>
    </owl:NamedIndividual>
    


    <!-- http://purl.obolibrary.org/obo/GAZ_00023301 -->

    <owl:NamedIndividual rdf:about="http://purl.obolibrary.org/obo/GAZ_00023301">
        <obo:RO_0001025 rdf:resource="http://purl.obolibrary.org/obo/GAZ_00014089"/>
        <obo:IAO_0000115>A large, mainly ice-covered island, 75 miles long and 20 miles wide, lying at the north side of Marguerite Bay off the west coast of the Antarctic Peninsula.</obo:IAO_0000115>
        <oboInOwl:hasOBONamespace>GAZ</oboInOwl:hasOBONamespace>
        <oboInOwl:id>GAZ:00023301</oboInOwl:id>
        <rdfs:label>Adelaide Island</rdfs:label>
    </owl:NamedIndividual>
    


    <!-- http://purl.obolibrary.org/obo/GAZ_00023302 -->

    <owl:NamedIndividual rdf:about="http://purl.obolibrary.org/obo/GAZ_00023302">
        <obo:RO_0001025 rdf:resource="http://purl.obolibrary.org/obo/GAZ_00023301"/>
        <obo:IAO_0000115>Point at the E side of the entrance to Ryder Bay, on the SE coast of Adelaide Island.</obo:IAO_0000115>
        <oboInOwl:hasOBONamespace>GAZ</oboInOwl:hasOBONamespace>
        <oboInOwl:id>GAZ:00023302</oboInOwl:id>
        <rdfs:label>Rothera Point</rdfs:label>
    </owl:NamedIndividual>
    


    <!-- http://purl.obolibrary.org/obo/GAZ_00023303 -->

    <owl:NamedIndividual rdf:about="http://purl.obolibrary.org/obo/GAZ_00023303">
        <obo:RO_0001025 rdf:resource="http://purl.obolibrary.org/obo/GAZ_00023304"/>
        <obo:IAO_0000115>A large bay which is bounded by Cape Johnson and Aviator Glacier Tongue on the north and Cape Washington on the south, along the coast of Victoria Land.</obo:IAO_0000115>
        <oboInOwl:hasOBONamespace>GAZ</oboInOwl:hasOBONamespace>
        <oboInOwl:id>GAZ:00023303</oboInOwl:id>
        <rdfs:label>Wood Bay</rdfs:label>
    </owl:NamedIndividual>
    


    <!-- http://purl.obolibrary.org/obo/GAZ_00023304 -->

    <owl:NamedIndividual rdf:about="http://purl.obolibrary.org/obo/GAZ_00023304">
        <rdf:type rdf:resource="http://purl.obolibrary.org/obo/ENVO_00000032"/>
        <obo:RO_0001025 rdf:resource="http://purl.obolibrary.org/obo/GAZ_00000373"/>
        <obo:IAO_0000115>A large embayment of the Southern Ocean, extending deeply into Antarctica between Cape Adare, at 170degE, on the west and Cape Colbeck on the east, at 158degW.</obo:IAO_0000115>
        <oboInOwl:hasOBONamespace>GAZ</oboInOwl:hasOBONamespace>
        <oboInOwl:id>GAZ:00023304</oboInOwl:id>
        <rdfs:label>Ross Sea</rdfs:label>
    </owl:NamedIndividual>
    


    <!-- http://purl.obolibrary.org/obo/GAZ_00023305 -->

    <owl:NamedIndividual rdf:about="http://purl.obolibrary.org/obo/GAZ_00023305">
        <obo:RO_0001025 rdf:resource="http://purl.obolibrary.org/obo/GAZ_00023304"/>
        <oboInOwl:hasOBONamespace>GAZ</oboInOwl:hasOBONamespace>
        <oboInOwl:id>GAZ:00023305</oboInOwl:id>
        <rdfs:label>Rod Bay</rdfs:label>
    </owl:NamedIndividual>
    


    <!-- http://purl.obolibrary.org/obo/GAZ_00023311 -->

    <owl:NamedIndividual rdf:about="http://purl.obolibrary.org/obo/GAZ_00023311">
        <obo:RO_0001025 rdf:resource="http://purl.obolibrary.org/obo/GAZ_00002625"/>
        <obo:IAO_0000115>A bay about 10 mi wide between Cape Bernacchi and Butter Point along the coast of Victoria Land.</obo:IAO_0000115>
        <oboInOwl:hasOBONamespace>GAZ</oboInOwl:hasOBONamespace>
        <oboInOwl:id>GAZ:00023311</oboInOwl:id>
        <rdfs:label>New Harbour</rdfs:label>
    </owl:NamedIndividual>
    


    <!-- http://purl.obolibrary.org/obo/GAZ_00023313 -->

    <owl:NamedIndividual rdf:about="http://purl.obolibrary.org/obo/GAZ_00023313">
        <obo:RO_0001025 rdf:resource="http://purl.obolibrary.org/obo/GAZ_00009005"/>
        <obo:IAO_0000115>An E-W ridge lying S of Cummings Cove in Signy Island, South Orkney Islands.</obo:IAO_0000115>
        <oboInOwl:hasOBONamespace>GAZ</oboInOwl:hasOBONamespace>
        <oboInOwl:id>GAZ:00023313</oboInOwl:id>
        <rdfs:label>Cryptogam Ridge</rdfs:label>
    </owl:NamedIndividual>
    


    <!-- http://purl.obolibrary.org/obo/GAZ_00023314 -->

    <owl:NamedIndividual rdf:about="http://purl.obolibrary.org/obo/GAZ_00023314">
        <obo:RO_0001025 rdf:resource="http://purl.obolibrary.org/obo/GAZ_00002625"/>
        <oboInOwl:hasOBONamespace>GAZ</oboInOwl:hasOBONamespace>
        <oboInOwl:id>GAZ:00023314</oboInOwl:id>
        <rdfs:label>McMurdo Jetty</rdfs:label>
    </owl:NamedIndividual>
    


    <!-- http://purl.obolibrary.org/obo/GAZ_00023315 -->

    <owl:NamedIndividual rdf:about="http://purl.obolibrary.org/obo/GAZ_00023315">
        <obo:RO_0001025 rdf:resource="http://purl.obolibrary.org/obo/GAZ_00023311"/>
        <obo:IAO_0000115>A cove at the northwest head of New Harbor, Victoria Land, on the west side of McMurdo Sound, where the Taylor Valley hits the seashore.</obo:IAO_0000115>
        <oboInOwl:hasOBONamespace>GAZ</oboInOwl:hasOBONamespace>
        <oboInOwl:id>GAZ:00023315</oboInOwl:id>
        <rdfs:label>Explorers Cove</rdfs:label>
    </owl:NamedIndividual>
    


    <!-- http://purl.obolibrary.org/obo/GAZ_00023316 -->

    <owl:NamedIndividual rdf:about="http://purl.obolibrary.org/obo/GAZ_00023316">
        <obo:RO_0001025 rdf:resource="http://purl.obolibrary.org/obo/GAZ_00004057"/>
        <obo:IAO_0000115>Rocky cape on the W side of Ross Island, forming the N side of the entrance to Erebus Bay.</obo:IAO_0000115>
        <oboInOwl:hasOBONamespace>GAZ</oboInOwl:hasOBONamespace>
        <oboInOwl:id>GAZ:00023316</oboInOwl:id>
        <rdfs:label>Cape Evans</rdfs:label>
    </owl:NamedIndividual>
    


    <!-- http://purl.obolibrary.org/obo/GAZ_00023318 -->

    <owl:NamedIndividual rdf:about="http://purl.obolibrary.org/obo/GAZ_00023318">
        <obo:RO_0001025 rdf:resource="http://purl.obolibrary.org/obo/GAZ_00009523"/>
        <obo:IAO_0000115>An island in the Antarctic Circle, the second largest of the South Orkney Islands.</obo:IAO_0000115>
        <oboInOwl:hasOBONamespace>GAZ</oboInOwl:hasOBONamespace>
        <oboInOwl:id>GAZ:00023318</oboInOwl:id>
        <rdfs:label>Laurie Island</rdfs:label>
    </owl:NamedIndividual>
    


    <!-- http://purl.obolibrary.org/obo/GAZ_00023319 -->

    <owl:NamedIndividual rdf:about="http://purl.obolibrary.org/obo/GAZ_00023319">
        <obo:RO_0001025 rdf:resource="http://purl.obolibrary.org/obo/GAZ_00009523"/>
        <obo:IAO_0000115>The largest of the South Orkney Islands.</obo:IAO_0000115>
        <oboInOwl:hasOBONamespace>GAZ</oboInOwl:hasOBONamespace>
        <oboInOwl:id>GAZ:00023319</oboInOwl:id>
        <rdfs:label>Coronation Island</rdfs:label>
    </owl:NamedIndividual>
    


    <!-- http://purl.obolibrary.org/obo/GAZ_00023320 -->

    <owl:NamedIndividual rdf:about="http://purl.obolibrary.org/obo/GAZ_00023320">
        <obo:RO_0001025 rdf:resource="http://purl.obolibrary.org/obo/GAZ_00009523"/>
        <obo:IAO_0000115>A narrow island 7 miles long and 2 miles wide, lying between Coronation and Laurie Islands in the central part of the South Orkney Islands.</obo:IAO_0000115>
        <oboInOwl:hasOBONamespace>GAZ</oboInOwl:hasOBONamespace>
        <oboInOwl:id>GAZ:00023320</oboInOwl:id>
        <rdfs:label>Powell Island</rdfs:label>
    </owl:NamedIndividual>
    


    <!-- http://purl.obolibrary.org/obo/GAZ_00023321 -->

    <owl:NamedIndividual rdf:about="http://purl.obolibrary.org/obo/GAZ_00023321">
        <obo:RO_0001025 rdf:resource="http://purl.obolibrary.org/obo/GAZ_00009523"/>
        <obo:IAO_0000115>A small island lying in the entrance to the bay on the E side of Matthews Island in the Robertson Islands group of the South Orkney Islands.</obo:IAO_0000115>
        <oboInOwl:hasOBONamespace>GAZ</oboInOwl:hasOBONamespace>
        <oboInOwl:id>GAZ:00023321</oboInOwl:id>
        <rdfs:label>Coffer Island</rdfs:label>
    </owl:NamedIndividual>
    


    <!-- http://purl.obolibrary.org/obo/GAZ_00023322 -->

    <owl:NamedIndividual rdf:about="http://purl.obolibrary.org/obo/GAZ_00023322">
        <obo:RO_0001025 rdf:resource="http://purl.obolibrary.org/obo/GAZ_00009523"/>
        <obo:IAO_0000115>An ice-covered island, 13 miles long in a northwest-southeast direction and 6 miles wide, lying at the east end of the Seal Nunataks off the east coast of the Antarctic Peninsula.</obo:IAO_0000115>
        <oboInOwl:hasOBONamespace>GAZ</oboInOwl:hasOBONamespace>
        <oboInOwl:id>GAZ:00023322</oboInOwl:id>
        <rdfs:label>Robertson Island</rdfs:label>
    </owl:NamedIndividual>
    


    <!-- http://purl.obolibrary.org/obo/GAZ_00023323 -->

    <owl:NamedIndividual rdf:about="http://purl.obolibrary.org/obo/GAZ_00023323">
        <obo:RO_0001025 rdf:resource="http://purl.obolibrary.org/obo/GAZ_00009523"/>
        <obo:IAO_0000115>An island nearly 3.2 km long, consisting of twin summits which are almost separated by a narrow channel strewn with boulders, lying 9 km north of the west end of Laurie Island in the South Orkney Islands.</obo:IAO_0000115>
        <oboInOwl:hasOBONamespace>GAZ</oboInOwl:hasOBONamespace>
        <oboInOwl:id>GAZ:00023323</oboInOwl:id>
        <rdfs:label>Saddle Island</rdfs:label>
    </owl:NamedIndividual>
    


    <!-- http://purl.obolibrary.org/obo/GAZ_00023324 -->

    <owl:NamedIndividual rdf:about="http://purl.obolibrary.org/obo/GAZ_00023324">
        <obo:RO_0001025 rdf:resource="http://purl.obolibrary.org/obo/GAZ_00009523"/>
        <obo:IAO_0000115>A group of small precipituous islands ranging from 120 to 215 m high, the westernmost features of the South Orkney Islands, lying 20 miles west of Coronation Island.</obo:IAO_0000115>
        <oboInOwl:hasOBONamespace>GAZ</oboInOwl:hasOBONamespace>
        <oboInOwl:id>GAZ:00023324</oboInOwl:id>
        <rdfs:label>Inaccessible Islands</rdfs:label>
    </owl:NamedIndividual>
    


    <!-- http://purl.obolibrary.org/obo/GAZ_00023325 -->

    <owl:NamedIndividual rdf:about="http://purl.obolibrary.org/obo/GAZ_00023325">
        <obo:RO_0001025 rdf:resource="http://purl.obolibrary.org/obo/GAZ_00009523"/>
        <obo:IAO_0000115>A small group of islands lying 1 mi NW of Moreton Point the W extremity of Coronation Island, in the South Orkney Islands.</obo:IAO_0000115>
        <oboInOwl:hasOBONamespace>GAZ</oboInOwl:hasOBONamespace>
        <oboInOwl:id>GAZ:00023325</oboInOwl:id>
        <rdfs:label>Larsen Islands</rdfs:label>
    </owl:NamedIndividual>
    


    <!-- http://purl.obolibrary.org/obo/GAZ_00023326 -->

    <owl:NamedIndividual rdf:about="http://purl.obolibrary.org/obo/GAZ_00023326">
        <obo:RO_0001025 rdf:resource="http://purl.obolibrary.org/obo/GAZ_00023334"/>
        <obo:IAO_0000115>A Chinese research station in Antarctica. It is located on King George Island. It is 2.5 km from the Chilean Frei Montalva Station, and 960 km from Cape Horn.</obo:IAO_0000115>
        <oboInOwl:hasOBONamespace>GAZ</oboInOwl:hasOBONamespace>
        <oboInOwl:id>GAZ:00023326</oboInOwl:id>
        <rdfs:label>Great Wall Station</rdfs:label>
    </owl:NamedIndividual>
    


    <!-- http://purl.obolibrary.org/obo/GAZ_00023328 -->

    <owl:NamedIndividual rdf:about="http://purl.obolibrary.org/obo/GAZ_00023328">
        <obo:RO_0001025 rdf:resource="http://purl.obolibrary.org/obo/GAZ_00051522"/>
        <obo:IAO_0000115>A French scientific station located in Antarctica on Ile des Petrels, archipelago of Pointe Geologie. Estabished 1956.</obo:IAO_0000115>
        <oboInOwl:hasOBONamespace>GAZ</oboInOwl:hasOBONamespace>
        <oboInOwl:id>GAZ:00023328</oboInOwl:id>
        <rdfs:label>Dumont d&apos;Urville Station</rdfs:label>
    </owl:NamedIndividual>
    


    <!-- http://purl.obolibrary.org/obo/GAZ_00023329 -->

    <owl:NamedIndividual rdf:about="http://purl.obolibrary.org/obo/GAZ_00023329">
        <obo:RO_0001025 rdf:resource="http://purl.obolibrary.org/obo/GAZ_00139422"/>
        <obo:IAO_0000115>A bay with a very narrow entrance in the northern part of the Vestfold Hills.</obo:IAO_0000115>
        <oboInOwl:hasOBONamespace>GAZ</oboInOwl:hasOBONamespace>
        <oboInOwl:id>GAZ:00023329</oboInOwl:id>
        <rdfs:label>Snezhnyy Bay</rdfs:label>
    </owl:NamedIndividual>
    


    <!-- http://purl.obolibrary.org/obo/GAZ_00023331 -->

    <owl:NamedIndividual rdf:about="http://purl.obolibrary.org/obo/GAZ_00023331">
        <obo:RO_0001025 rdf:resource="http://purl.obolibrary.org/obo/GAZ_00023303"/>
        <obo:IAO_0000115>A rounded, largely ice-free point lying below Mount Melbourne along the W side of Wood Bay, Victoria Land.</obo:IAO_0000115>
        <oboInOwl:hasOBONamespace>GAZ</oboInOwl:hasOBONamespace>
        <oboInOwl:id>GAZ:00023331</oboInOwl:id>
        <rdfs:label>Edmonson Point</rdfs:label>
    </owl:NamedIndividual>
    


    <!-- http://purl.obolibrary.org/obo/GAZ_00023332 -->

    <owl:NamedIndividual rdf:about="http://purl.obolibrary.org/obo/GAZ_00023332">
        <obo:RO_0001025 rdf:resource="http://purl.obolibrary.org/obo/GAZ_00139422"/>
        <obo:IAO_0000115>A narrow inlet about 33 km long, between Mule Peninsula and Broad Peninsula in the Vestfold Hills on the Ingrid Christensen Coast.</obo:IAO_0000115>
        <oboInOwl:hasOBONamespace>GAZ</oboInOwl:hasOBONamespace>
        <oboInOwl:id>GAZ:00023332</oboInOwl:id>
        <rdfs:label>Ellis Fjord</rdfs:label>
    </owl:NamedIndividual>
    


    <!-- http://purl.obolibrary.org/obo/GAZ_00023333 -->

    <owl:NamedIndividual rdf:about="http://purl.obolibrary.org/obo/GAZ_00023333">
        <obo:RO_0001025 rdf:resource="http://purl.obolibrary.org/obo/GAZ_00011782"/>
        <obo:IAO_0000115>A cove in Terra Nova Bay, Victoria Lan, entered between Inexpressible Island and Cape Russell.</obo:IAO_0000115>
        <oboInOwl:hasOBONamespace>GAZ</oboInOwl:hasOBONamespace>
        <oboInOwl:id>GAZ:00023333</oboInOwl:id>
        <rdfs:label>Evans Cove</rdfs:label>
    </owl:NamedIndividual>
    


    <!-- http://purl.obolibrary.org/obo/GAZ_00023334 -->

    <owl:NamedIndividual rdf:about="http://purl.obolibrary.org/obo/GAZ_00023334">
        <obo:RO_0001025 rdf:resource="http://purl.obolibrary.org/obo/GAZ_00007425"/>
        <obo:IAO_0000115>A peninsula in thw SW extremity of King George Island, 7 km long.</obo:IAO_0000115>
        <oboInOwl:hasOBONamespace>GAZ</oboInOwl:hasOBONamespace>
        <oboInOwl:id>GAZ:00023334</oboInOwl:id>
        <rdfs:label>Fildes Peninsula</rdfs:label>
    </owl:NamedIndividual>
    


    <!-- http://purl.obolibrary.org/obo/GAZ_00023336 -->

    <owl:NamedIndividual rdf:about="http://purl.obolibrary.org/obo/GAZ_00023336">
        <obo:RO_0001025 rdf:resource="http://purl.obolibrary.org/obo/GAZ_00014122"/>
        <oboInOwl:hasOBONamespace>GAZ</oboInOwl:hasOBONamespace>
        <oboInOwl:id>GAZ:00023336</oboInOwl:id>
        <rdfs:label>Irizar Island</rdfs:label>
    </owl:NamedIndividual>
    


    <!-- http://purl.obolibrary.org/obo/GAZ_00023337 -->

    <owl:NamedIndividual rdf:about="http://purl.obolibrary.org/obo/GAZ_00023337">
        <obo:RO_0001025 rdf:resource="http://purl.obolibrary.org/obo/GAZ_00014122"/>
        <obo:IAO_0000115>An island in the Wilhelm Archipelago.</obo:IAO_0000115>
        <oboInOwl:hasOBONamespace>GAZ</oboInOwl:hasOBONamespace>
        <oboInOwl:id>GAZ:00023337</oboInOwl:id>
        <rdfs:label>Booth Island</rdfs:label>
    </owl:NamedIndividual>
    


    <!-- http://purl.obolibrary.org/obo/GAZ_00023338 -->

    <owl:NamedIndividual rdf:about="http://purl.obolibrary.org/obo/GAZ_00023338">
        <obo:RO_0001025 rdf:resource="http://purl.obolibrary.org/obo/GAZ_00014122"/>
        <obo:IAO_0000115>An island 4.8 km long, lying 2.4 km southwest of Booth Island in the Wilhelm Archipelago.</obo:IAO_0000115>
        <oboInOwl:hasOBONamespace>GAZ</oboInOwl:hasOBONamespace>
        <oboInOwl:id>GAZ:00023338</oboInOwl:id>
        <rdfs:label>Hovgaard Island</rdfs:label>
    </owl:NamedIndividual>
    


    <!-- http://purl.obolibrary.org/obo/GAZ_00023339 -->

    <owl:NamedIndividual rdf:about="http://purl.obolibrary.org/obo/GAZ_00023339">
        <obo:RO_0001025 rdf:resource="http://purl.obolibrary.org/obo/GAZ_00023303"/>
        <obo:IAO_0000115>A small island lying 2 mi E of Cape Johnson in the N part of Wood Bay, Victoria Land.</obo:IAO_0000115>
        <oboInOwl:hasOBONamespace>GAZ</oboInOwl:hasOBONamespace>
        <oboInOwl:id>GAZ:00023339</oboInOwl:id>
        <rdfs:label>Kay Island</rdfs:label>
    </owl:NamedIndividual>
    


    <!-- http://purl.obolibrary.org/obo/GAZ_00023340 -->

    <owl:NamedIndividual rdf:about="http://purl.obolibrary.org/obo/GAZ_00023340">
        <obo:RO_0001025 rdf:resource="http://purl.obolibrary.org/obo/GAZ_00004045"/>
        <obo:IAO_0000115>An ice-covered island, 13 miles long in a northwest-southeast direction and 6 miles wide, lying at the east end of the Seal Nunataks off the east coast of the Antarctic Peninsula.</obo:IAO_0000115>
        <oboInOwl:hasOBONamespace>GAZ</oboInOwl:hasOBONamespace>
        <oboInOwl:id>GAZ:00023340</oboInOwl:id>
        <rdfs:label>Leonie Island</rdfs:label>
    </owl:NamedIndividual>
    


    <!-- http://purl.obolibrary.org/obo/GAZ_00023342 -->

    <owl:NamedIndividual rdf:about="http://purl.obolibrary.org/obo/GAZ_00023342">
        <obo:RO_0001025 rdf:resource="http://purl.obolibrary.org/obo/GAZ_00140059"/>
        <obo:IAO_0000115>A bay 10 mi long, lying between King George Island and Nelson Island, in the South Shetland Islands.</obo:IAO_0000115>
        <oboInOwl:hasOBONamespace>GAZ</oboInOwl:hasOBONamespace>
        <oboInOwl:id>GAZ:00023342</oboInOwl:id>
        <rdfs:label>Maxwell Bay</rdfs:label>
    </owl:NamedIndividual>
    


    <!-- http://purl.obolibrary.org/obo/GAZ_00023343 -->

    <owl:NamedIndividual rdf:about="http://purl.obolibrary.org/obo/GAZ_00023343">
        <obo:RO_0001025 rdf:resource="http://purl.obolibrary.org/obo/GAZ_00002625"/>
        <obo:IAO_0000115>That part of the Ross Ice Shelf bounded by McMurdo Sound and Ross Island on the north and Minna Bluff on the south. Studies show this feature has characteristics quite distinct from the Ross Ice Shelf and merits individual naming.</obo:IAO_0000115>
        <oboInOwl:hasOBONamespace>GAZ</oboInOwl:hasOBONamespace>
        <oboInOwl:id>GAZ:00023343</oboInOwl:id>
        <rdfs:label>McMurdo Ice Shelf</rdfs:label>
    </owl:NamedIndividual>
    


    <!-- http://purl.obolibrary.org/obo/GAZ_00023344 -->

    <owl:NamedIndividual rdf:about="http://purl.obolibrary.org/obo/GAZ_00023344">
        <obo:RO_0001025 rdf:resource="http://purl.obolibrary.org/obo/GAZ_00023343"/>
        <oboInOwl:hasOBONamespace>GAZ</oboInOwl:hasOBONamespace>
        <oboInOwl:id>GAZ:00023344</oboInOwl:id>
        <rdfs:label>Orange Pond</rdfs:label>
    </owl:NamedIndividual>
    


    <!-- http://purl.obolibrary.org/obo/GAZ_00023345 -->

    <owl:NamedIndividual rdf:about="http://purl.obolibrary.org/obo/GAZ_00023345">
        <obo:RO_0001025 rdf:resource="http://purl.obolibrary.org/obo/GAZ_00023343"/>
        <oboInOwl:hasOBONamespace>GAZ</oboInOwl:hasOBONamespace>
        <oboInOwl:id>GAZ:00023345</oboInOwl:id>
        <rdfs:label>Salt Pond</rdfs:label>
    </owl:NamedIndividual>
    


    <!-- http://purl.obolibrary.org/obo/GAZ_00023346 -->

    <owl:NamedIndividual rdf:about="http://purl.obolibrary.org/obo/GAZ_00023346">
        <obo:RO_0001025 rdf:resource="http://purl.obolibrary.org/obo/GAZ_00011769"/>
        <obo:IAO_0000115>An ice dome approximately 100 km wide and 100 km long, located 130 km east of Siple Coast.</obo:IAO_0000115>
        <oboInOwl:hasOBONamespace>GAZ</oboInOwl:hasOBONamespace>
        <oboInOwl:id>GAZ:00023346</oboInOwl:id>
        <rdfs:label>Siple Dome</rdfs:label>
    </owl:NamedIndividual>
    


    <!-- http://purl.obolibrary.org/obo/GAZ_00023348 -->

    <owl:NamedIndividual rdf:about="http://purl.obolibrary.org/obo/GAZ_00023348">
        <obo:RO_0001025 rdf:resource="http://purl.obolibrary.org/obo/GAZ_00140059"/>
        <obo:IAO_0000115>A strait about 60 miles wide extending for 200 miles in a general northeast-southwest direction between the South Shetland Islands and Antarctic Peninsula.</obo:IAO_0000115>
        <oboInOwl:hasOBONamespace>GAZ</oboInOwl:hasOBONamespace>
        <oboInOwl:id>GAZ:00023348</oboInOwl:id>
        <rdfs:label>Bransfield Strait</rdfs:label>
    </owl:NamedIndividual>
    


    <!-- http://purl.obolibrary.org/obo/GAZ_00023349 -->

    <owl:NamedIndividual rdf:about="http://purl.obolibrary.org/obo/GAZ_00023349">
        <obo:RO_0001025 rdf:resource="http://purl.obolibrary.org/obo/GAZ_00023348"/>
        <obo:IAO_0000115>An island 3 mi long, lying in Bransfield Strait 14 mi NW of Cape Ducorps, Trinity Peninsula.</obo:IAO_0000115>
        <oboInOwl:hasOBONamespace>GAZ</oboInOwl:hasOBONamespace>
        <oboInOwl:id>GAZ:00023349</oboInOwl:id>
        <rdfs:label>Astrolabe Island</rdfs:label>
    </owl:NamedIndividual>
    


    <!-- http://purl.obolibrary.org/obo/GAZ_00023350 -->

    <owl:NamedIndividual rdf:about="http://purl.obolibrary.org/obo/GAZ_00023350">
        <obo:RO_0001025 rdf:resource="http://purl.obolibrary.org/obo/GAZ_00004380"/>
        <obo:IAO_0000115>Monolith rising c. 50 m above sea level off Claude Point, Brabant Island.</obo:IAO_0000115>
        <oboInOwl:hasOBONamespace>GAZ</oboInOwl:hasOBONamespace>
        <oboInOwl:id>GAZ:00023350</oboInOwl:id>
        <rdfs:label>Astrolabe Needle</rdfs:label>
    </owl:NamedIndividual>
    


    <!-- http://purl.obolibrary.org/obo/GAZ_00023352 -->

    <owl:NamedIndividual rdf:about="http://purl.obolibrary.org/obo/GAZ_00023352">
        <obo:RO_0001025 rdf:resource="http://purl.obolibrary.org/obo/GAZ_00051499"/>
        <obo:IAO_0000115>Small archipelago of rocky islands and rocks close N of Cape Geodesie and Astrolabe Glacier Tongue, extending from Helene Island on the W to Dumoulin Islands on the east.</obo:IAO_0000115>
        <oboInOwl:hasOBONamespace>GAZ</oboInOwl:hasOBONamespace>
        <oboInOwl:id>GAZ:00023352</oboInOwl:id>
        <rdfs:label>Geologie Archipelago</rdfs:label>
    </owl:NamedIndividual>
    


    <!-- http://purl.obolibrary.org/obo/GAZ_00023357 -->

    <owl:NamedIndividual rdf:about="http://purl.obolibrary.org/obo/GAZ_00023357">
        <obo:RO_0001025 rdf:resource="http://purl.obolibrary.org/obo/GAZ_00011782"/>
        <obo:IAO_0000115>A rock cape in Terra Nova Bay along the coast of Victoria Land, forming the S extremity of the Northern Foothills.</obo:IAO_0000115>
        <oboInOwl:hasOBONamespace>GAZ</oboInOwl:hasOBONamespace>
        <oboInOwl:id>GAZ:00023357</oboInOwl:id>
        <rdfs:label>Cap Russell</rdfs:label>
    </owl:NamedIndividual>
    


    <!-- http://purl.obolibrary.org/obo/GAZ_00023358 -->

    <owl:NamedIndividual rdf:about="http://purl.obolibrary.org/obo/GAZ_00023358">
        <obo:RO_0001025 rdf:resource="http://purl.obolibrary.org/obo/GAZ_00004057"/>
        <obo:IAO_0000115>A long, narrow land mass from 4.8 km wide and 24 km long, projecting southwest from the slopes of Mount Erebus on Ross Island.</obo:IAO_0000115>
        <oboInOwl:hasOBONamespace>GAZ</oboInOwl:hasOBONamespace>
        <oboInOwl:id>GAZ:00023358</oboInOwl:id>
        <rdfs:label>Hut Point Peninsula</rdfs:label>
    </owl:NamedIndividual>
    


    <!-- http://purl.obolibrary.org/obo/GAZ_00023359 -->

    <owl:NamedIndividual rdf:about="http://purl.obolibrary.org/obo/GAZ_00023359">
        <obo:RO_0001025 rdf:resource="http://purl.obolibrary.org/obo/GAZ_00023358"/>
        <obo:IAO_0000115>A Cape forming the S end of Hut Point Peninsula and the southernmost point on Ross Island.</obo:IAO_0000115>
        <oboInOwl:hasOBONamespace>GAZ</oboInOwl:hasOBONamespace>
        <oboInOwl:id>GAZ:00023359</oboInOwl:id>
        <rdfs:label>Cape Armitage</rdfs:label>
    </owl:NamedIndividual>
    


    <!-- http://purl.obolibrary.org/obo/GAZ_00023362 -->

    <owl:NamedIndividual rdf:about="http://purl.obolibrary.org/obo/GAZ_00023362">
        <obo:RO_0001025 rdf:resource="http://purl.obolibrary.org/obo/GAZ_00023304"/>
        <obo:IAO_0000115>A cove.</obo:IAO_0000115>
        <oboInOwl:hasOBONamespace>GAZ</oboInOwl:hasOBONamespace>
        <oboInOwl:id>GAZ:00023362</oboInOwl:id>
        <rdfs:label>Adelie Cove</rdfs:label>
    </owl:NamedIndividual>
    


    <!-- http://purl.obolibrary.org/obo/GAZ_00023363 -->

    <owl:NamedIndividual rdf:about="http://purl.obolibrary.org/obo/GAZ_00023363">
        <obo:RO_0001025 rdf:resource="http://purl.obolibrary.org/obo/GAZ_00014099"/>
        <obo:IAO_0000115>A small rocky island, the northernmost of the Dellbridge Islands, lying 1 mile southwest of Cape Evans, Ross Island.</obo:IAO_0000115>
        <oboInOwl:hasOBONamespace>GAZ</oboInOwl:hasOBONamespace>
        <oboInOwl:id>GAZ:00023363</oboInOwl:id>
        <rdfs:label>Inaccessible Island</rdfs:label>
    </owl:NamedIndividual>
    


    <!-- http://purl.obolibrary.org/obo/GAZ_00023364 -->

    <owl:NamedIndividual rdf:about="http://purl.obolibrary.org/obo/GAZ_00023364">
        <obo:RO_0001025 rdf:resource="http://purl.obolibrary.org/obo/GAZ_00014099"/>
        <obo:IAO_0000115>One of the Dellbridge Islands in McMurdo Sound, Antarctica.</obo:IAO_0000115>
        <oboInOwl:hasOBONamespace>GAZ</oboInOwl:hasOBONamespace>
        <oboInOwl:id>GAZ:00023364</oboInOwl:id>
        <rdfs:label>Tent Island</rdfs:label>
    </owl:NamedIndividual>
    


    <!-- http://purl.obolibrary.org/obo/GAZ_00023365 -->

    <owl:NamedIndividual rdf:about="http://purl.obolibrary.org/obo/GAZ_00023365">
        <obo:RO_0001025 rdf:resource="http://purl.obolibrary.org/obo/GAZ_00014099"/>
        <obo:IAO_0000115>The smallest and easternmost of the Dellbridge Islands, lying in Erebus Bay off the W side of Ross Island.</obo:IAO_0000115>
        <oboInOwl:hasOBONamespace>GAZ</oboInOwl:hasOBONamespace>
        <oboInOwl:id>GAZ:00023365</oboInOwl:id>
        <rdfs:label>Little Razorback Island</rdfs:label>
    </owl:NamedIndividual>
    


    <!-- http://purl.obolibrary.org/obo/GAZ_00023366 -->

    <owl:NamedIndividual rdf:about="http://purl.obolibrary.org/obo/GAZ_00023366">
        <obo:RO_0001025 rdf:resource="http://purl.obolibrary.org/obo/GAZ_00014099"/>
        <obo:IAO_0000115>The southeasternmost of the Dellbridge Islands, lying in Erebus Bay off the W side of Ross Island.</obo:IAO_0000115>
        <oboInOwl:hasOBONamespace>GAZ</oboInOwl:hasOBONamespace>
        <oboInOwl:id>GAZ:00023366</oboInOwl:id>
        <rdfs:label>Big Razorback Island</rdfs:label>
    </owl:NamedIndividual>
    


    <!-- http://purl.obolibrary.org/obo/GAZ_00044998 -->

    <owl:NamedIndividual rdf:about="http://purl.obolibrary.org/obo/GAZ_00044998">
        <obo:RO_0001025 rdf:resource="http://purl.obolibrary.org/obo/GAZ_00045057"/>
        <obo:IAO_0000115>An open bay, 10 mi wide at its entrance between Adams Island and the Haswell Islands, lying immediately W of Mabus Point on the coast of Antarctica.</obo:IAO_0000115>
        <oboInOwl:hasOBONamespace>GAZ</oboInOwl:hasOBONamespace>
        <oboInOwl:id>GAZ:00044998</oboInOwl:id>
        <rdfs:label>McDonald Bay</rdfs:label>
    </owl:NamedIndividual>
    


    <!-- http://purl.obolibrary.org/obo/GAZ_00044999 -->

    <owl:NamedIndividual rdf:about="http://purl.obolibrary.org/obo/GAZ_00044999">
        <obo:RO_0001025 rdf:resource="http://purl.obolibrary.org/obo/GAZ_00044998"/>
        <obo:IAO_0000115>Asmall rocky coastal sub-antarctic island embedded in thick bay ice most of the year, lying at the western side of McDonald Bay, about 17 km west of Mabus Point.</obo:IAO_0000115>
        <oboInOwl:hasOBONamespace>GAZ</oboInOwl:hasOBONamespace>
        <oboInOwl:id>GAZ:00044999</oboInOwl:id>
        <rdfs:label>Adams Island</rdfs:label>
    </owl:NamedIndividual>
    


    <!-- http://purl.obolibrary.org/obo/GAZ_00045000 -->

    <owl:NamedIndividual rdf:about="http://purl.obolibrary.org/obo/GAZ_00045000">
        <obo:RO_0001025 rdf:resource="http://purl.obolibrary.org/obo/GAZ_00051499"/>
        <obo:IAO_0000115>A chain of uninhabited, mainly volcanic, islands in the Southern Ocean stretching from 66deg15min to 67deg35minS and 162deg30min to 165deg00minE. The group forms a chain that extends for about 160 km in a northwest-southeast direction. The islands are heavily glaciated and are of volcanic origin. Ice tongues project from their slopes into the sea. The islands were formed by the Balleny hotspot.</obo:IAO_0000115>
        <oboInOwl:hasOBONamespace>GAZ</oboInOwl:hasOBONamespace>
        <oboInOwl:id>GAZ:00045000</oboInOwl:id>
        <rdfs:label>Balleny Islands</rdfs:label>
    </owl:NamedIndividual>
    


    <!-- http://purl.obolibrary.org/obo/GAZ_00045001 -->

    <owl:NamedIndividual rdf:about="http://purl.obolibrary.org/obo/GAZ_00045001">
        <obo:RO_0001025 rdf:resource="http://purl.obolibrary.org/obo/GAZ_00045002"/>
        <oboInOwl:hasOBONamespace>GAZ</oboInOwl:hasOBONamespace>
        <oboInOwl:id>GAZ:00045001</oboInOwl:id>
        <rdfs:label>Eliza Cone</rdfs:label>
    </owl:NamedIndividual>
    


    <!-- http://purl.obolibrary.org/obo/GAZ_00045002 -->

    <owl:NamedIndividual rdf:about="http://purl.obolibrary.org/obo/GAZ_00045002">
        <obo:RO_0001025 rdf:resource="http://purl.obolibrary.org/obo/GAZ_00045000"/>
        <oboInOwl:hasOBONamespace>GAZ</oboInOwl:hasOBONamespace>
        <oboInOwl:id>GAZ:00045002</oboInOwl:id>
        <rdfs:label>Buckle Islands</rdfs:label>
    </owl:NamedIndividual>
    


    <!-- http://purl.obolibrary.org/obo/GAZ_00045003 -->

    <owl:NamedIndividual rdf:about="http://purl.obolibrary.org/obo/GAZ_00045003">
        <obo:RO_0001025 rdf:resource="http://purl.obolibrary.org/obo/GAZ_00045000"/>
        <oboInOwl:hasOBONamespace>GAZ</oboInOwl:hasOBONamespace>
        <oboInOwl:id>GAZ:00045003</oboInOwl:id>
        <rdfs:label>Young Islands</rdfs:label>
    </owl:NamedIndividual>
    


    <!-- http://purl.obolibrary.org/obo/GAZ_00045004 -->

    <owl:NamedIndividual rdf:about="http://purl.obolibrary.org/obo/GAZ_00045004">
        <obo:RO_0001025 rdf:resource="http://purl.obolibrary.org/obo/GAZ_00045002"/>
        <oboInOwl:hasOBONamespace>GAZ</oboInOwl:hasOBONamespace>
        <oboInOwl:id>GAZ:00045004</oboInOwl:id>
        <rdfs:label>The Monolith</rdfs:label>
    </owl:NamedIndividual>
    


    <!-- http://purl.obolibrary.org/obo/GAZ_00045005 -->

    <owl:NamedIndividual rdf:about="http://purl.obolibrary.org/obo/GAZ_00045005">
        <obo:RO_0001025 rdf:resource="http://purl.obolibrary.org/obo/GAZ_00045003"/>
        <obo:IAO_0000115>An ice-covered island betwen Buckle Island and Young Island.</obo:IAO_0000115>
        <oboInOwl:hasOBONamespace>GAZ</oboInOwl:hasOBONamespace>
        <oboInOwl:id>GAZ:00045005</oboInOwl:id>
        <rdfs:label>Borradaile Island</rdfs:label>
    </owl:NamedIndividual>
    


    <!-- http://purl.obolibrary.org/obo/GAZ_00045006 -->

    <owl:NamedIndividual rdf:about="http://purl.obolibrary.org/obo/GAZ_00045006">
        <obo:RO_0001025 rdf:resource="http://purl.obolibrary.org/obo/GAZ_00045003"/>
        <oboInOwl:hasOBONamespace>GAZ</oboInOwl:hasOBONamespace>
        <oboInOwl:id>GAZ:00045006</oboInOwl:id>
        <rdfs:label>Pillar</rdfs:label>
    </owl:NamedIndividual>
    


    <!-- http://purl.obolibrary.org/obo/GAZ_00045007 -->

    <owl:NamedIndividual rdf:about="http://purl.obolibrary.org/obo/GAZ_00045007">
        <obo:RO_0001025 rdf:resource="http://purl.obolibrary.org/obo/GAZ_00045003"/>
        <obo:IAO_0000115>The northernmost and westernmost of the three main islands in the uninhabited Balleny Islands group located in the Southern Ocean. It lies eight km northwest of Buckle Island, some 115 km north-northeast of Belousov Point on the Antarctic mainland.</obo:IAO_0000115>
        <oboInOwl:hasOBONamespace>GAZ</oboInOwl:hasOBONamespace>
        <oboInOwl:id>GAZ:00045007</oboInOwl:id>
        <rdfs:label>Young Island</rdfs:label>
    </owl:NamedIndividual>
    


    <!-- http://purl.obolibrary.org/obo/GAZ_00045008 -->

    <owl:NamedIndividual rdf:about="http://purl.obolibrary.org/obo/GAZ_00045008">
        <obo:RO_0001025 rdf:resource="http://purl.obolibrary.org/obo/GAZ_00045003"/>
        <obo:IAO_0000115>Rocks near Young Island.</obo:IAO_0000115>
        <oboInOwl:hasOBONamespace>GAZ</oboInOwl:hasOBONamespace>
        <oboInOwl:id>GAZ:00045008</oboInOwl:id>
        <rdfs:label>Seal Rocks</rdfs:label>
    </owl:NamedIndividual>
    


    <!-- http://purl.obolibrary.org/obo/GAZ_00045009 -->

    <owl:NamedIndividual rdf:about="http://purl.obolibrary.org/obo/GAZ_00045009">
        <obo:RO_0001025 rdf:resource="http://purl.obolibrary.org/obo/GAZ_00045003"/>
        <oboInOwl:hasOBONamespace>GAZ</oboInOwl:hasOBONamespace>
        <oboInOwl:id>GAZ:00045009</oboInOwl:id>
        <rdfs:label>Row Island</rdfs:label>
    </owl:NamedIndividual>
    


    <!-- http://purl.obolibrary.org/obo/GAZ_00045010 -->

    <owl:NamedIndividual rdf:about="http://purl.obolibrary.org/obo/GAZ_00045010">
        <obo:RO_0001025 rdf:resource="http://purl.obolibrary.org/obo/GAZ_00045003"/>
        <oboInOwl:hasOBONamespace>GAZ</oboInOwl:hasOBONamespace>
        <oboInOwl:id>GAZ:00045010</oboInOwl:id>
        <rdfs:label>Beale Pinnacle</rdfs:label>
    </owl:NamedIndividual>
    


    <!-- http://purl.obolibrary.org/obo/GAZ_00045011 -->

    <owl:NamedIndividual rdf:about="http://purl.obolibrary.org/obo/GAZ_00045011">
        <obo:RO_0001025 rdf:resource="http://purl.obolibrary.org/obo/GAZ_00045002"/>
        <obo:IAO_0000115>A satellite island of Buckle Island.</obo:IAO_0000115>
        <oboInOwl:hasOBONamespace>GAZ</oboInOwl:hasOBONamespace>
        <oboInOwl:id>GAZ:00045011</oboInOwl:id>
        <rdfs:label>Chinstrap Islet</rdfs:label>
    </owl:NamedIndividual>
    


    <!-- http://purl.obolibrary.org/obo/GAZ_00045012 -->

    <owl:NamedIndividual rdf:about="http://purl.obolibrary.org/obo/GAZ_00045012">
        <obo:RO_0001025 rdf:resource="http://purl.obolibrary.org/obo/GAZ_00045002"/>
        <obo:IAO_0000115>The largest of three small islets lying 1 mile southward of Buckle Island in the Balleny Islands.</obo:IAO_0000115>
        <oboInOwl:hasOBONamespace>GAZ</oboInOwl:hasOBONamespace>
        <oboInOwl:id>GAZ:00045012</oboInOwl:id>
        <rdfs:label>Sabrina Island</rdfs:label>
    </owl:NamedIndividual>
    


    <!-- http://purl.obolibrary.org/obo/GAZ_00045013 -->

    <owl:NamedIndividual rdf:about="http://purl.obolibrary.org/obo/GAZ_00045013">
        <obo:RO_0001025 rdf:resource="http://purl.obolibrary.org/obo/GAZ_00045002"/>
        <oboInOwl:hasOBONamespace>GAZ</oboInOwl:hasOBONamespace>
        <oboInOwl:id>GAZ:00045013</oboInOwl:id>
        <rdfs:label>Scott Cone</rdfs:label>
    </owl:NamedIndividual>
    


    <!-- http://purl.obolibrary.org/obo/GAZ_00045014 -->

    <owl:NamedIndividual rdf:about="http://purl.obolibrary.org/obo/GAZ_00045014">
        <obo:RO_0001025 rdf:resource="http://purl.obolibrary.org/obo/GAZ_00045002"/>
        <obo:IAO_0000115>One of the three main islands in the uninhabited Balleny Islands group located in the Southern Ocean. It lies 25 km northwest of Sturge Island and eight km southeast of Young Island, some 110 km north-northeast of Belousov Point on the Antarctic mainland. Dark eruption columns were reported during 1839 and 1899, but no detailed geological studies exist for Balleny Islands volcanoes.</obo:IAO_0000115>
        <oboInOwl:hasOBONamespace>GAZ</oboInOwl:hasOBONamespace>
        <oboInOwl:id>GAZ:00045014</oboInOwl:id>
        <rdfs:label>Buckle Island</rdfs:label>
    </owl:NamedIndividual>
    


    <!-- http://purl.obolibrary.org/obo/GAZ_00045015 -->

    <owl:NamedIndividual rdf:about="http://purl.obolibrary.org/obo/GAZ_00045015">
        <obo:RO_0001025 rdf:resource="http://purl.obolibrary.org/obo/GAZ_00045000"/>
        <obo:IAO_0000115>One of the three main islands in the uninhabited Balleny Islands group located in the Southern Ocean. It lies 25 km southeast of Buckle Island and 95 km northeast of Belousov Point on the Antarctic mainland.</obo:IAO_0000115>
        <oboInOwl:hasOBONamespace>GAZ</oboInOwl:hasOBONamespace>
        <oboInOwl:id>GAZ:00045015</oboInOwl:id>
        <rdfs:label>Sturge Island</rdfs:label>
    </owl:NamedIndividual>
    


    <!-- http://purl.obolibrary.org/obo/GAZ_00045016 -->

    <owl:NamedIndividual rdf:about="http://purl.obolibrary.org/obo/GAZ_00045016">
        <obo:RO_0001025 rdf:resource="http://purl.obolibrary.org/obo/GAZ_00014089"/>
        <obo:IAO_0000115>An island 1.5 miles long which rises to 675 m, lying 1 mile northwest of Roman Four Promontory and directly north of the mouth of Neny Fjord, off the west coast of Graham Land in Antarctica.</obo:IAO_0000115>
        <oboInOwl:hasOBONamespace>GAZ</oboInOwl:hasOBONamespace>
        <oboInOwl:id>GAZ:00045016</oboInOwl:id>
        <rdfs:label>Neny Island</rdfs:label>
    </owl:NamedIndividual>
    


    <!-- http://purl.obolibrary.org/obo/GAZ_00045017 -->

    <owl:NamedIndividual rdf:about="http://purl.obolibrary.org/obo/GAZ_00045017">
        <obo:RO_0001025 rdf:resource="http://purl.obolibrary.org/obo/GAZ_00014089"/>
        <obo:IAO_0000115>A rocky island lying 1 mile northeast of Neny Island in the eastern part of Marguerite Bay, off the west coast of Graham Land.</obo:IAO_0000115>
        <oboInOwl:hasOBONamespace>GAZ</oboInOwl:hasOBONamespace>
        <oboInOwl:id>GAZ:00045017</oboInOwl:id>
        <rdfs:label>Stonington Island</rdfs:label>
    </owl:NamedIndividual>
    


    <!-- http://purl.obolibrary.org/obo/GAZ_00045018 -->

    <owl:NamedIndividual rdf:about="http://purl.obolibrary.org/obo/GAZ_00045018">
        <obo:RO_0001025 rdf:resource="http://purl.obolibrary.org/obo/GAZ_00014089"/>
        <obo:IAO_0000115>A rocky island lying 1 mile west of Stonington Island in Marguerite Bay, off the coast of Graham Land.</obo:IAO_0000115>
        <oboInOwl:hasOBONamespace>GAZ</oboInOwl:hasOBONamespace>
        <oboInOwl:id>GAZ:00045018</oboInOwl:id>
        <rdfs:label>Bear Island</rdfs:label>
    </owl:NamedIndividual>
    


    <!-- http://purl.obolibrary.org/obo/GAZ_00045019 -->

    <owl:NamedIndividual rdf:about="http://purl.obolibrary.org/obo/GAZ_00045019">
        <obo:RO_0001025 rdf:resource="http://purl.obolibrary.org/obo/GAZ_00141552"/>
        <obo:IAO_0000115>A bay 15 miles wide between Reclus Peninsula and Cape Anna along the west coast of Graham Land.</obo:IAO_0000115>
        <oboInOwl:hasOBONamespace>GAZ</oboInOwl:hasOBONamespace>
        <oboInOwl:id>GAZ:00045019</oboInOwl:id>
        <rdfs:label>Wilhelmina Bay</rdfs:label>
    </owl:NamedIndividual>
    


    <!-- http://purl.obolibrary.org/obo/GAZ_00045020 -->

    <owl:NamedIndividual rdf:about="http://purl.obolibrary.org/obo/GAZ_00045020">
        <obo:RO_0001025 rdf:resource="http://purl.obolibrary.org/obo/GAZ_00045019"/>
        <obo:IAO_0000115>A small antarctic island lying midway between Nansen Island and Enterprise Island in Wilhelmina Bay, off the west coast of Graham Land.</obo:IAO_0000115>
        <oboInOwl:hasOBONamespace>GAZ</oboInOwl:hasOBONamespace>
        <oboInOwl:id>GAZ:00045020</oboInOwl:id>
        <rdfs:label>Bearing Island</rdfs:label>
    </owl:NamedIndividual>
    


    <!-- http://purl.obolibrary.org/obo/GAZ_00045021 -->

    <owl:NamedIndividual rdf:about="http://purl.obolibrary.org/obo/GAZ_00045021">
        <obo:RO_0001025 rdf:resource="http://purl.obolibrary.org/obo/GAZ_00045019"/>
        <oboInOwl:hasOBONamespace>GAZ</oboInOwl:hasOBONamespace>
        <oboInOwl:id>GAZ:00045021</oboInOwl:id>
        <rdfs:label>Nansen Island</rdfs:label>
    </owl:NamedIndividual>
    


    <!-- http://purl.obolibrary.org/obo/GAZ_00045022 -->

    <owl:NamedIndividual rdf:about="http://purl.obolibrary.org/obo/GAZ_00045022">
        <obo:RO_0001025 rdf:resource="http://purl.obolibrary.org/obo/GAZ_00045019"/>
        <obo:IAO_0000115>An island off the NE coast of Nansen Island.</obo:IAO_0000115>
        <oboInOwl:hasOBONamespace>GAZ</oboInOwl:hasOBONamespace>
        <oboInOwl:id>GAZ:00045022</oboInOwl:id>
        <rdfs:label>Enterprise Island</rdfs:label>
    </owl:NamedIndividual>
    


    <!-- http://purl.obolibrary.org/obo/GAZ_00045023 -->

    <owl:NamedIndividual rdf:about="http://purl.obolibrary.org/obo/GAZ_00045023">
        <obo:RO_0001025 rdf:resource="http://purl.obolibrary.org/obo/GAZ_00004045"/>
        <obo:IAO_0000115>A high and completely ice-covered island about 320 km long and 135 km wide in Antarctica, with an area of 43873.1 km2.</obo:IAO_0000115>
        <oboInOwl:hasOBONamespace>GAZ</oboInOwl:hasOBONamespace>
        <oboInOwl:id>GAZ:00045023</oboInOwl:id>
        <rdfs:label>Berkner Island</rdfs:label>
    </owl:NamedIndividual>
    


    <!-- http://purl.obolibrary.org/obo/GAZ_00045024 -->

    <owl:NamedIndividual rdf:about="http://purl.obolibrary.org/obo/GAZ_00045024">
        <obo:RO_0001025 rdf:resource="http://purl.obolibrary.org/obo/GAZ_00141552"/>
        <obo:IAO_0000115>A chain of islands, of which the principal ones are Renaud, Rabot, Lavoisier (named Serrano by Chile and Mitre by Argentina) and Watkins, lying parallel to the W coast of Graham Land and extending 80 miles in a NE-SW direction.</obo:IAO_0000115>
        <oboInOwl:hasOBONamespace>GAZ</oboInOwl:hasOBONamespace>
        <oboInOwl:id>GAZ:00045024</oboInOwl:id>
        <rdfs:label>Biscoe Islands</rdfs:label>
    </owl:NamedIndividual>
    


    <!-- http://purl.obolibrary.org/obo/GAZ_00045025 -->

    <owl:NamedIndividual rdf:about="http://purl.obolibrary.org/obo/GAZ_00045025">
        <obo:RO_0001025 rdf:resource="http://purl.obolibrary.org/obo/GAZ_00045024"/>
        <obo:IAO_0000115>Una isla baja cubierta por el hielo, de unas 5 millas de largo por unas 3 millas de ancho, al suroeste de la isla Lavoisier en el archipielago de las islas Biscoe en la Antartida.</obo:IAO_0000115>
        <oboInOwl:hasOBONamespace>GAZ</oboInOwl:hasOBONamespace>
        <oboInOwl:id>GAZ:00045025</oboInOwl:id>
        <rdfs:label>Watkins Island</rdfs:label>
    </owl:NamedIndividual>
    


    <!-- http://purl.obolibrary.org/obo/GAZ_00045026 -->

    <owl:NamedIndividual rdf:about="http://purl.obolibrary.org/obo/GAZ_00045026">
        <obo:RO_0001025 rdf:resource="http://purl.obolibrary.org/obo/GAZ_00045024"/>
        <obo:IAO_0000115>Una isla perteneciente a las Islas Biscoe, archipielago adyacente a la costa occidental de la Peninsula Antartica. La Isla Rabot se ubica al sur de la Isla Renaud (la mayor del grupo), de la cual esta separada por un estrecho canal (1.5 km aprox). Rabot mide alrededor de 8 km de largo por 3 km de ancho.</obo:IAO_0000115>
        <oboInOwl:hasOBONamespace>GAZ</oboInOwl:hasOBONamespace>
        <oboInOwl:id>GAZ:00045026</oboInOwl:id>
        <rdfs:label>Rabot Island</rdfs:label>
    </owl:NamedIndividual>
    


    <!-- http://purl.obolibrary.org/obo/GAZ_00045027 -->

    <owl:NamedIndividual rdf:about="http://purl.obolibrary.org/obo/GAZ_00045027">
        <obo:RO_0001025 rdf:resource="http://purl.obolibrary.org/obo/GAZ_00045024"/>
        <obo:IAO_0000115>La mayor de las Islas Biscoe, adyacente a la costa occidental de la Peninsula Antartica. La isla se ubica entre las Islas Pitt, hacia el norte; la Isla Rabot al sureste, separadas por el Paso Covadonga; y la Isla Lavoisier (llamada Serrano por Chile y Mitre por Argentina) al sur, separadas por el Estrecho Pendleton.</obo:IAO_0000115>
        <oboInOwl:hasOBONamespace>GAZ</oboInOwl:hasOBONamespace>
        <oboInOwl:id>GAZ:00045027</oboInOwl:id>
        <rdfs:label>Renaud Island</rdfs:label>
    </owl:NamedIndividual>
    


    <!-- http://purl.obolibrary.org/obo/GAZ_00045028 -->

    <owl:NamedIndividual rdf:about="http://purl.obolibrary.org/obo/GAZ_00045028">
        <obo:RO_0001025 rdf:resource="http://purl.obolibrary.org/obo/GAZ_00045024"/>
        <obo:IAO_0000115>La segunda en extension de las Islas Biscoe, archipielago adyacente a la costa oeste de la Peninsula Antartica. Lavoisier se ubica entre la Isla Renaud y la Isla Rabot al noreste, separadas por el Estrecho Pendleton; y la Isla Watkins al suroeste.</obo:IAO_0000115>
        <oboInOwl:hasOBONamespace>GAZ</oboInOwl:hasOBONamespace>
        <oboInOwl:id>GAZ:00045028</oboInOwl:id>
        <rdfs:label>Lavoisier Island</rdfs:label>
    </owl:NamedIndividual>
    


    <!-- http://purl.obolibrary.org/obo/GAZ_00045029 -->

    <owl:NamedIndividual rdf:about="http://purl.obolibrary.org/obo/GAZ_00045029">
        <obo:RO_0001025 rdf:resource="http://purl.obolibrary.org/obo/GAZ_00045074"/>
        <obo:IAO_0000115>A high ice-covered island, about 24 mi long and from 2 to 6 mi wide, shaped like a figure eight. The feature rises above the NE part of Shackleton Ice Shelf, which partially encloses the island, 25 mi NE of Cape Elliott.</obo:IAO_0000115>
        <oboInOwl:hasOBONamespace>GAZ</oboInOwl:hasOBONamespace>
        <oboInOwl:id>GAZ:00045029</oboInOwl:id>
        <rdfs:label>Bowman Island</rdfs:label>
    </owl:NamedIndividual>
    


    <!-- http://purl.obolibrary.org/obo/GAZ_00045030 -->

    <owl:NamedIndividual rdf:about="http://purl.obolibrary.org/obo/GAZ_00045030">
        <obo:RO_0001025 rdf:resource="http://purl.obolibrary.org/obo/GAZ_00004380"/>
        <obo:IAO_0000115>An ice-covered island. Second largest of the Palmer Archipelago.</obo:IAO_0000115>
        <oboInOwl:hasOBONamespace>GAZ</oboInOwl:hasOBONamespace>
        <oboInOwl:id>GAZ:00045030</oboInOwl:id>
        <rdfs:label>Brabant Island</rdfs:label>
    </owl:NamedIndividual>
    


    <!-- http://purl.obolibrary.org/obo/GAZ_00045031 -->

    <owl:NamedIndividual rdf:about="http://purl.obolibrary.org/obo/GAZ_00045031">
        <obo:RO_0001025 rdf:resource="http://purl.obolibrary.org/obo/GAZ_00004380"/>
        <obo:IAO_0000115>An island, 9 miles long and 3 miles wide, lying immediately northeast of Brabant Island in the Palmer Archipelago.</obo:IAO_0000115>
        <oboInOwl:hasOBONamespace>GAZ</oboInOwl:hasOBONamespace>
        <oboInOwl:id>GAZ:00045031</oboInOwl:id>
        <rdfs:label>Liege Island</rdfs:label>
    </owl:NamedIndividual>
    


    <!-- http://purl.obolibrary.org/obo/GAZ_00045032 -->

    <owl:NamedIndividual rdf:about="http://purl.obolibrary.org/obo/GAZ_00045032">
        <obo:RO_0001025 rdf:resource="http://purl.obolibrary.org/obo/GAZ_00004380"/>
        <obo:IAO_0000115>A small rocky island off Antarctica lying close southwest of Norsel Point, off the southwest coast of Anvers Island in the Palmer Archipelago.</obo:IAO_0000115>
        <oboInOwl:hasOBONamespace>GAZ</oboInOwl:hasOBONamespace>
        <oboInOwl:id>GAZ:00045032</oboInOwl:id>
        <rdfs:label>Breaker Island</rdfs:label>
    </owl:NamedIndividual>
    


    <!-- http://purl.obolibrary.org/obo/GAZ_00045033 -->

    <owl:NamedIndividual rdf:about="http://purl.obolibrary.org/obo/GAZ_00045033">
        <obo:RO_0001025 rdf:resource="http://purl.obolibrary.org/obo/GAZ_00014085"/>
        <obo:IAO_0000115>An ice-covered island about 16 miles long and 6 miles wide, lying 37 miles southwest of Cape Waite, King Peninsula, in the Amundsen Sea.</obo:IAO_0000115>
        <oboInOwl:hasOBONamespace>GAZ</oboInOwl:hasOBONamespace>
        <oboInOwl:id>GAZ:00045033</oboInOwl:id>
        <rdfs:label>Burke Island</rdfs:label>
    </owl:NamedIndividual>
    


    <!-- http://purl.obolibrary.org/obo/GAZ_00045034 -->

    <owl:NamedIndividual rdf:about="http://purl.obolibrary.org/obo/GAZ_00045034">
        <rdf:type rdf:resource="http://purl.obolibrary.org/obo/ENVO_00000032"/>
        <obo:RO_0001025 rdf:resource="http://purl.obolibrary.org/obo/GAZ_00141555"/>
        <obo:IAO_0000115>A long embayment 24 miles wide, close west of the Tula Mountains in Enderby Land, Antarctica.</obo:IAO_0000115>
        <oboInOwl:hasOBONamespace>GAZ</oboInOwl:hasOBONamespace>
        <oboInOwl:id>GAZ:00045034</oboInOwl:id>
        <rdfs:label>Amundsen Bay</rdfs:label>
    </owl:NamedIndividual>
    


    <!-- http://purl.obolibrary.org/obo/GAZ_00045035 -->

    <owl:NamedIndividual rdf:about="http://purl.obolibrary.org/obo/GAZ_00045035">
        <obo:RO_0001025 rdf:resource="http://purl.obolibrary.org/obo/GAZ_00045034"/>
        <obo:IAO_0000115>A group of small islands lying just west of Mount Gleadell in the eastern part of Amundsen Bay, in Enderby Land.</obo:IAO_0000115>
        <oboInOwl:hasOBONamespace>GAZ</oboInOwl:hasOBONamespace>
        <oboInOwl:id>GAZ:00045035</oboInOwl:id>
        <rdfs:label>Burkett Islands</rdfs:label>
    </owl:NamedIndividual>
    


    <!-- http://purl.obolibrary.org/obo/GAZ_00045041 -->

    <owl:NamedIndividual rdf:about="http://purl.obolibrary.org/obo/GAZ_00045041">
        <obo:RO_0001025 rdf:resource="http://purl.obolibrary.org/obo/GAZ_00014085"/>
        <obo:RO_0001025 rdf:resource="http://purl.obolibrary.org/obo/GAZ_00141556"/>
        <obo:IAO_0000115>An Antarctic ice shelf, over 480 km long and from 32 to 96 km wide, bordering the Hobbs and Bakutis Coasts of Marie Byrd Land between McDonald Heights and Martin Peninsula. Several large islands are partially or wholly embedded in the ice shelf.</obo:IAO_0000115>
        <oboInOwl:hasOBONamespace>GAZ</oboInOwl:hasOBONamespace>
        <oboInOwl:id>GAZ:00045041</oboInOwl:id>
        <rdfs:label>Getz Ice Shelf</rdfs:label>
    </owl:NamedIndividual>
    


    <!-- http://purl.obolibrary.org/obo/GAZ_00045042 -->

    <owl:NamedIndividual rdf:about="http://purl.obolibrary.org/obo/GAZ_00045042">
        <obo:RO_0001025 rdf:resource="http://purl.obolibrary.org/obo/GAZ_00045041"/>
        <obo:IAO_0000115>An ice-covered island, 110 km long and about 8,500 km2 in area, with all but its North coast lying within the Getz Ice Shelf, Antarctica. It is located between Siple Island and Wright Island along the coast of Marie Byrd Land.</obo:IAO_0000115>
        <oboInOwl:hasOBONamespace>GAZ</oboInOwl:hasOBONamespace>
        <oboInOwl:id>GAZ:00045042</oboInOwl:id>
        <rdfs:label>Carney Island</rdfs:label>
    </owl:NamedIndividual>
    


    <!-- http://purl.obolibrary.org/obo/GAZ_00045043 -->

    <owl:NamedIndividual rdf:about="http://purl.obolibrary.org/obo/GAZ_00045043">
        <obo:RO_0001025 rdf:resource="http://purl.obolibrary.org/obo/GAZ_00014085"/>
        <obo:IAO_0000115>An ice-covered island 60 km long, lying at the north edge of Getz Ice Shelf about midway between Carney Island and Martin Peninsula, on the Bakutis Coast, Marie Byrd Land.</obo:IAO_0000115>
        <oboInOwl:hasOBONamespace>GAZ</oboInOwl:hasOBONamespace>
        <oboInOwl:id>GAZ:00045043</oboInOwl:id>
        <rdfs:label>Wright Island</rdfs:label>
    </owl:NamedIndividual>
    


    <!-- http://purl.obolibrary.org/obo/GAZ_00045044 -->

    <owl:NamedIndividual rdf:about="http://purl.obolibrary.org/obo/GAZ_00045044">
        <obo:RO_0001025 rdf:resource="http://purl.obolibrary.org/obo/GAZ_00045041"/>
        <obo:IAO_0000115>A 110 km long snow-covered island lying east of Wrigley Gulf along the Getz Ice Shelf off Bakutis Coast of Marie Byrd Land, Antarctica.</obo:IAO_0000115>
        <oboInOwl:hasOBONamespace>GAZ</oboInOwl:hasOBONamespace>
        <oboInOwl:id>GAZ:00045044</oboInOwl:id>
        <rdfs:label>Siple Island</rdfs:label>
    </owl:NamedIndividual>
    


    <!-- http://purl.obolibrary.org/obo/GAZ_00045045 -->

    <owl:NamedIndividual rdf:about="http://purl.obolibrary.org/obo/GAZ_00045045">
        <obo:RO_0001025 rdf:resource="http://purl.obolibrary.org/obo/GAZ_00004380"/>
        <obo:IAO_0000115>An island 0.5 mi long which lies 1 mile off the south coast of Anvers Island and 1.5 miles southeast of Bonaparte Point.</obo:IAO_0000115>
        <oboInOwl:hasOBONamespace>GAZ</oboInOwl:hasOBONamespace>
        <oboInOwl:id>GAZ:00045045</oboInOwl:id>
        <rdfs:label>Christine Island</rdfs:label>
    </owl:NamedIndividual>
    


    <!-- http://purl.obolibrary.org/obo/GAZ_00045046 -->

    <owl:NamedIndividual rdf:about="http://purl.obolibrary.org/obo/GAZ_00045046">
        <obo:RO_0001025 rdf:resource="http://purl.obolibrary.org/obo/GAZ_00004380"/>
        <obo:IAO_0000115>An island lying off the south side of Anvers Island, 2.5 miles East-southeast of Bonaparte Point, in the Palmer Archipelago.</obo:IAO_0000115>
        <oboInOwl:hasOBONamespace>GAZ</oboInOwl:hasOBONamespace>
        <oboInOwl:id>GAZ:00045046</oboInOwl:id>
        <rdfs:label>Cormorant Island</rdfs:label>
    </owl:NamedIndividual>
    


    <!-- http://purl.obolibrary.org/obo/GAZ_00045047 -->

    <owl:NamedIndividual rdf:about="http://purl.obolibrary.org/obo/GAZ_00045047">
        <obo:RO_0001025 rdf:resource="http://purl.obolibrary.org/obo/GAZ_00023304"/>
        <obo:IAO_0000115>An ice-covered island, composed of several connected shield volcanos in the Ross Sea off Antarctica. The Coulman caldera, 5 km wide and 700 m deep, can be found on the south end of the island.</obo:IAO_0000115>
        <oboInOwl:hasOBONamespace>GAZ</oboInOwl:hasOBONamespace>
        <oboInOwl:id>GAZ:00045047</oboInOwl:id>
        <rdfs:label>Coulman Island</rdfs:label>
    </owl:NamedIndividual>
    


    <!-- http://purl.obolibrary.org/obo/GAZ_00045048 -->

    <owl:NamedIndividual rdf:about="http://purl.obolibrary.org/obo/GAZ_00045048">
        <obo:RO_0001025 rdf:resource="http://purl.obolibrary.org/obo/GAZ_00141552"/>
        <obo:IAO_0000115>A dark, rocky island lying in Errera Channel between Arctowski Peninsula and the northern part of Ronge Island, off the west coast of Graham Land.</obo:IAO_0000115>
        <oboInOwl:hasOBONamespace>GAZ</oboInOwl:hasOBONamespace>
        <oboInOwl:id>GAZ:00045048</oboInOwl:id>
        <rdfs:label>Cuverville Island</rdfs:label>
    </owl:NamedIndividual>
    


    <!-- http://purl.obolibrary.org/obo/GAZ_00045049 -->

    <owl:NamedIndividual rdf:about="http://purl.obolibrary.org/obo/GAZ_00045049">
        <obo:RO_0001025 rdf:resource="http://purl.obolibrary.org/obo/GAZ_00141552"/>
        <obo:IAO_0000115>An island off Antarctica, 1 mile long lying in the southern part of Errera Channel, off the west coast of Graham Land.</obo:IAO_0000115>
        <oboInOwl:hasOBONamespace>GAZ</oboInOwl:hasOBONamespace>
        <oboInOwl:id>GAZ:00045049</oboInOwl:id>
        <rdfs:label>Danco Island</rdfs:label>
    </owl:NamedIndividual>
    


    <!-- http://purl.obolibrary.org/obo/GAZ_00045050 -->

    <owl:NamedIndividual rdf:about="http://purl.obolibrary.org/obo/GAZ_00045050">
        <obo:RO_0001025 rdf:resource="http://purl.obolibrary.org/obo/GAZ_00141552"/>
        <obo:IAO_0000115>A group of islands and rocks lying between Millerand Island and the west coast of Graham Land.</obo:IAO_0000115>
        <oboInOwl:hasOBONamespace>GAZ</oboInOwl:hasOBONamespace>
        <oboInOwl:id>GAZ:00045050</oboInOwl:id>
        <rdfs:label>Debenham Islands</rdfs:label>
    </owl:NamedIndividual>
    


    <!-- http://purl.obolibrary.org/obo/GAZ_00045051 -->

    <owl:NamedIndividual rdf:about="http://purl.obolibrary.org/obo/GAZ_00045051">
        <obo:RO_0001025 rdf:resource="http://purl.obolibrary.org/obo/GAZ_00045050"/>
        <obo:IAO_0000115>An island lying in the centre of the Debenham Islands, off the west coast of Graham Land.</obo:IAO_0000115>
        <oboInOwl:hasOBONamespace>GAZ</oboInOwl:hasOBONamespace>
        <oboInOwl:id>GAZ:00045051</oboInOwl:id>
        <rdfs:label>Barry Island</rdfs:label>
    </owl:NamedIndividual>
    


    <!-- http://purl.obolibrary.org/obo/GAZ_00045052 -->

    <owl:NamedIndividual rdf:about="http://purl.obolibrary.org/obo/GAZ_00045052">
        <obo:RO_0001025 rdf:resource="http://purl.obolibrary.org/obo/GAZ_00004380"/>
        <obo:IAO_0000115>A small U-shaped island 0.8 miles west of Bonaparte Point, off the southwest coast of Anvers Island.</obo:IAO_0000115>
        <oboInOwl:hasOBONamespace>GAZ</oboInOwl:hasOBONamespace>
        <oboInOwl:id>GAZ:00045052</oboInOwl:id>
        <rdfs:label>DeLaca Island</rdfs:label>
    </owl:NamedIndividual>
    


    <!-- http://purl.obolibrary.org/obo/GAZ_00045054 -->

    <owl:NamedIndividual rdf:about="http://purl.obolibrary.org/obo/GAZ_00045054">
        <obo:RO_0001025 rdf:resource="http://purl.obolibrary.org/obo/GAZ_00004380"/>
        <obo:IAO_0000115>A small island between Anvers Island and Wienke Islands.</obo:IAO_0000115>
        <oboInOwl:hasOBONamespace>GAZ</oboInOwl:hasOBONamespace>
        <oboInOwl:id>GAZ:00045054</oboInOwl:id>
        <rdfs:label>Doumer Island</rdfs:label>
    </owl:NamedIndividual>
    


    <!-- http://purl.obolibrary.org/obo/GAZ_00045055 -->

    <owl:NamedIndividual rdf:about="http://purl.obolibrary.org/obo/GAZ_00045055">
        <obo:RO_0001025 rdf:resource="http://purl.obolibrary.org/obo/GAZ_00004380"/>
        <obo:IAO_0000115>An island 16 miles long and from 2 to 5 miles wide, about 67 km in area, the southernmost of the major islands of the Palmer Archipelago, lying between Anvers Island to its north and the west coast of the Antarctic Peninsula.</obo:IAO_0000115>
        <oboInOwl:hasOBONamespace>GAZ</oboInOwl:hasOBONamespace>
        <oboInOwl:id>GAZ:00045055</oboInOwl:id>
        <rdfs:label>Wiencke Island</rdfs:label>
    </owl:NamedIndividual>
    


    <!-- http://purl.obolibrary.org/obo/GAZ_00045056 -->

    <owl:NamedIndividual rdf:about="http://purl.obolibrary.org/obo/GAZ_00045056">
        <obo:RO_0001025 rdf:resource="http://purl.obolibrary.org/obo/GAZ_00004380"/>
        <obo:IAO_0000115>An island lying 1 mile southeast of Cape Monaco, off the southwest coast of Anvers Island in the Palmer Archipelago.</obo:IAO_0000115>
        <oboInOwl:hasOBONamespace>GAZ</oboInOwl:hasOBONamespace>
        <oboInOwl:id>GAZ:00045056</oboInOwl:id>
        <rdfs:label>Dream Island</rdfs:label>
    </owl:NamedIndividual>
    


    <!-- http://purl.obolibrary.org/obo/GAZ_00045057 -->

    <owl:NamedIndividual rdf:about="http://purl.obolibrary.org/obo/GAZ_00045057">
        <obo:RO_0001025 rdf:resource="http://purl.obolibrary.org/obo/GAZ_00000373"/>
        <obo:IAO_0000115>A coastal sea along the coast of Antarctica between West Ice Shelf, at approximately 80deg E, and E end of the Shackleton Ice Shelf, at approximately 105degE. No definitive N boundary.</obo:IAO_0000115>
        <oboInOwl:hasOBONamespace>GAZ</oboInOwl:hasOBONamespace>
        <oboInOwl:id>GAZ:00045057</oboInOwl:id>
        <rdfs:label>Davis Sea</rdfs:label>
    </owl:NamedIndividual>
    


    <!-- http://purl.obolibrary.org/obo/GAZ_00045058 -->

    <owl:NamedIndividual rdf:about="http://purl.obolibrary.org/obo/GAZ_00045058">
        <obo:RO_0001025 rdf:resource="http://purl.obolibrary.org/obo/GAZ_00045057"/>
        <obo:IAO_0000115>An ice-capped island with a dome about 327 m high that is 11 miles long and rises to 325 m in the Davis Sea of the Southern Ocean about 85 km north of the coast of Queen Mary Land and 45 miles north-northeast (NNE) of Cape Filchner.</obo:IAO_0000115>
        <oboInOwl:hasOBONamespace>GAZ</oboInOwl:hasOBONamespace>
        <oboInOwl:id>GAZ:00045058</oboInOwl:id>
        <rdfs:label>Drygalski Island</rdfs:label>
    </owl:NamedIndividual>
    


    <!-- http://purl.obolibrary.org/obo/GAZ_00045059 -->

    <owl:NamedIndividual rdf:about="http://purl.obolibrary.org/obo/GAZ_00045059">
        <obo:RO_0001025 rdf:resource="http://purl.obolibrary.org/obo/GAZ_00004380"/>
        <obo:IAO_0000115>A small island whose west end is deeply cleft into three parts, giving the appearance of three separate rocks at high tide, lying between Shortcut Island and Surge Rocks off the southwest coast of Anvers Island.</obo:IAO_0000115>
        <oboInOwl:hasOBONamespace>GAZ</oboInOwl:hasOBONamespace>
        <oboInOwl:id>GAZ:00045059</oboInOwl:id>
        <rdfs:label>Eichorst Island</rdfs:label>
    </owl:NamedIndividual>
    


    <!-- http://purl.obolibrary.org/obo/GAZ_00045060 -->

    <owl:NamedIndividual rdf:about="http://purl.obolibrary.org/obo/GAZ_00045060">
        <obo:RO_0001025 rdf:resource="http://purl.obolibrary.org/obo/GAZ_00004380"/>
        <obo:IAO_0000115>A crescent-shaped island 0.4 miles long, with three prominent indentations of the north shore, lying 0.7 miles SSE of Gamage Point and Palmer Station along the SW coast of Anvers Island.</obo:IAO_0000115>
        <oboInOwl:hasOBONamespace>GAZ</oboInOwl:hasOBONamespace>
        <oboInOwl:id>GAZ:00045060</oboInOwl:id>
        <rdfs:label>Shortcut Island</rdfs:label>
    </owl:NamedIndividual>
    


    <!-- http://purl.obolibrary.org/obo/GAZ_00045061 -->

    <owl:NamedIndividual rdf:about="http://purl.obolibrary.org/obo/GAZ_00045061">
        <obo:RO_0001025 rdf:resource="http://purl.obolibrary.org/obo/GAZ_00004380"/>
        <obo:IAO_0000115>A group of five rocks, two always exposed, lying 0.1 miles southwest of Eichorst Island and 0.6 miles south-southeast of Bonaparte Point, Anvers Island.</obo:IAO_0000115>
        <oboInOwl:hasOBONamespace>GAZ</oboInOwl:hasOBONamespace>
        <oboInOwl:id>GAZ:00045061</oboInOwl:id>
        <rdfs:label>Surge Rocks</rdfs:label>
    </owl:NamedIndividual>
    


    <!-- http://purl.obolibrary.org/obo/GAZ_00045062 -->

    <owl:NamedIndividual rdf:about="http://purl.obolibrary.org/obo/GAZ_00045062">
        <obo:RO_0001025 rdf:resource="http://purl.obolibrary.org/obo/GAZ_00004380"/>
        <obo:IAO_0000115>A rocky island 0.5 miles long and rising to 50 m, lying 0.5 miles south of Norsel Point, off the southwest coast of Anvers Island in the Palmer Archipelago.</obo:IAO_0000115>
        <oboInOwl:hasOBONamespace>GAZ</oboInOwl:hasOBONamespace>
        <oboInOwl:id>GAZ:00045062</oboInOwl:id>
        <rdfs:label>Litchfield Island</rdfs:label>
    </owl:NamedIndividual>
    


    <!-- http://purl.obolibrary.org/obo/GAZ_00045063 -->

    <owl:NamedIndividual rdf:about="http://purl.obolibrary.org/obo/GAZ_00045063">
        <obo:RO_0001025 rdf:resource="http://purl.obolibrary.org/obo/GAZ_00004380"/>
        <obo:IAO_0000115>A group of three prominent rocks connected by shoals, located between Torgersen Island and the northwest entrance to Arthur Harbor, off the southwest coast of Anvers Island.</obo:IAO_0000115>
        <oboInOwl:hasOBONamespace>GAZ</oboInOwl:hasOBONamespace>
        <oboInOwl:id>GAZ:00045063</oboInOwl:id>
        <rdfs:label>Elephant Rocks</rdfs:label>
    </owl:NamedIndividual>
    


    <!-- http://purl.obolibrary.org/obo/GAZ_00045064 -->

    <owl:NamedIndividual rdf:about="http://purl.obolibrary.org/obo/GAZ_00045064">
        <obo:RO_0001025 rdf:resource="http://purl.obolibrary.org/obo/GAZ_00004380"/>
        <obo:IAO_0000115>A small rocky island lying just east of Litchfield Island in the entrance to Arthur Harbor, off the southwest coast of Anvers Island in the Palmer Archipelago.</obo:IAO_0000115>
        <oboInOwl:hasOBONamespace>GAZ</oboInOwl:hasOBONamespace>
        <oboInOwl:id>GAZ:00045064</oboInOwl:id>
        <rdfs:label>Torgersen Island</rdfs:label>
    </owl:NamedIndividual>
    


    <!-- http://purl.obolibrary.org/obo/GAZ_00045065 -->

    <owl:NamedIndividual rdf:about="http://purl.obolibrary.org/obo/GAZ_00045065">
        <obo:RO_0001025 rdf:resource="http://purl.obolibrary.org/obo/GAZ_00139422"/>
        <obo:IAO_0000115>A bay in Antarctica, 22 miles wide, containing many islands, indenting the coast 5 miles north of the Framnes Mountains.</obo:IAO_0000115>
        <oboInOwl:hasOBONamespace>GAZ</oboInOwl:hasOBONamespace>
        <oboInOwl:id>GAZ:00045065</oboInOwl:id>
        <rdfs:label>Holme Bay</rdfs:label>
    </owl:NamedIndividual>
    


    <!-- http://purl.obolibrary.org/obo/GAZ_00045066 -->

    <owl:NamedIndividual rdf:about="http://purl.obolibrary.org/obo/GAZ_00045066">
        <obo:RO_0001025 rdf:resource="http://purl.obolibrary.org/obo/GAZ_00045065"/>
        <obo:IAO_0000115>A small chain of islands which extends 2.5 miles in a northeast-southwest direction, lying about 3 km north-west of Mawson Station and 2 miles southwest of Welch Island in the eastern part of Holme Bay.</obo:IAO_0000115>
        <oboInOwl:hasOBONamespace>GAZ</oboInOwl:hasOBONamespace>
        <oboInOwl:id>GAZ:00045066</oboInOwl:id>
        <rdfs:label>Flat Islands</rdfs:label>
    </owl:NamedIndividual>
    


    <!-- http://purl.obolibrary.org/obo/GAZ_00045067 -->

    <owl:NamedIndividual rdf:about="http://purl.obolibrary.org/obo/GAZ_00045067">
        <obo:RO_0001025 rdf:resource="http://purl.obolibrary.org/obo/GAZ_00045065"/>
        <obo:IAO_0000115>An island, one mile long with a prominent pinnacle rock of 130 m, lying north of Rouse Islands and one mile off the shore in the eastern side of Holme Bay.</obo:IAO_0000115>
        <oboInOwl:hasOBONamespace>GAZ</oboInOwl:hasOBONamespace>
        <oboInOwl:id>GAZ:00045067</oboInOwl:id>
        <rdfs:label>Welch Island</rdfs:label>
    </owl:NamedIndividual>
    


    <!-- http://purl.obolibrary.org/obo/GAZ_00045068 -->

    <owl:NamedIndividual rdf:about="http://purl.obolibrary.org/obo/GAZ_00045068">
        <obo:RO_0001025 rdf:resource="http://purl.obolibrary.org/obo/GAZ_00045065"/>
        <obo:IAO_0000115>A small group of islands in the eastern part of Holme Bay, fringing the coast of Mac Robertson Land close south of Welch Island.</obo:IAO_0000115>
        <oboInOwl:hasOBONamespace>GAZ</oboInOwl:hasOBONamespace>
        <oboInOwl:id>GAZ:00045068</oboInOwl:id>
        <rdfs:label>Rouse Islands</rdfs:label>
    </owl:NamedIndividual>
    


    <!-- http://purl.obolibrary.org/obo/GAZ_00045069 -->

    <owl:NamedIndividual rdf:about="http://purl.obolibrary.org/obo/GAZ_00045069">
        <obo:RO_0001025 rdf:resource="http://purl.obolibrary.org/obo/GAZ_00045070"/>
        <obo:IAO_0000115>A rocky island, 0.4 km in diameter, which is the largest of the Fletcher Islands.</obo:IAO_0000115>
        <oboInOwl:hasOBONamespace>GAZ</oboInOwl:hasOBONamespace>
        <oboInOwl:id>GAZ:00045069</oboInOwl:id>
        <rdfs:label>Fletcher Island</rdfs:label>
    </owl:NamedIndividual>
    


    <!-- http://purl.obolibrary.org/obo/GAZ_00045070 -->

    <owl:NamedIndividual rdf:about="http://purl.obolibrary.org/obo/GAZ_00045070">
        <obo:RO_0001025 rdf:resource="http://purl.obolibrary.org/obo/GAZ_00023276"/>
        <obo:IAO_0000115>A small group of islands lying 6 miles west-southwest (WSW) of Cape Gray in the eastern part of Commonwealth Bay.</obo:IAO_0000115>
        <oboInOwl:hasOBONamespace>GAZ</oboInOwl:hasOBONamespace>
        <oboInOwl:id>GAZ:00045070</oboInOwl:id>
        <rdfs:label>Fletcher Islands</rdfs:label>
    </owl:NamedIndividual>
    


    <!-- http://purl.obolibrary.org/obo/GAZ_00045071 -->

    <owl:NamedIndividual rdf:about="http://purl.obolibrary.org/obo/GAZ_00045071">
        <obo:RO_0001025 rdf:resource="http://purl.obolibrary.org/obo/GAZ_00045041"/>
        <obo:IAO_0000115>An island about 11 miles long, lying 6 miles west of Grant Island off the coast of Marie Byrd Land.</obo:IAO_0000115>
        <oboInOwl:hasOBONamespace>GAZ</oboInOwl:hasOBONamespace>
        <oboInOwl:id>GAZ:00045071</oboInOwl:id>
        <rdfs:label>Shepard Island</rdfs:label>
    </owl:NamedIndividual>
    


    <!-- http://purl.obolibrary.org/obo/GAZ_00045072 -->

    <owl:NamedIndividual rdf:about="http://purl.obolibrary.org/obo/GAZ_00045072">
        <obo:RO_0001025 rdf:resource="http://purl.obolibrary.org/obo/GAZ_00045041"/>
        <obo:IAO_0000115>An ice-covered island, 20 mi long and 10 mi wide, lying 5 mi E of the smaller Shepard Island off the coast of Marie Byrd Land. Surrounded by the Getz Ice Shelf on all but the N side.</obo:IAO_0000115>
        <oboInOwl:hasOBONamespace>GAZ</oboInOwl:hasOBONamespace>
        <oboInOwl:id>GAZ:00045072</oboInOwl:id>
        <rdfs:label>Grant Island</rdfs:label>
    </owl:NamedIndividual>
    


    <!-- http://purl.obolibrary.org/obo/GAZ_00045073 -->

    <owl:NamedIndividual rdf:about="http://purl.obolibrary.org/obo/GAZ_00045073">
        <obo:RO_0001025 rdf:resource="http://purl.obolibrary.org/obo/GAZ_00004380"/>
        <obo:IAO_0000115>An island lying 2.5 miles northwest of Litchfield Island, off the southwest coast of Anvers Island in the Palmer Archipelago.</obo:IAO_0000115>
        <oboInOwl:hasOBONamespace>GAZ</oboInOwl:hasOBONamespace>
        <oboInOwl:id>GAZ:00045073</oboInOwl:id>
        <rdfs:label>Halfway Island</rdfs:label>
    </owl:NamedIndividual>
    


    <!-- http://purl.obolibrary.org/obo/GAZ_00045074 -->

    <owl:NamedIndividual rdf:about="http://purl.obolibrary.org/obo/GAZ_00045074">
        <obo:RO_0001025 rdf:resource="http://purl.obolibrary.org/obo/GAZ_00045057"/>
        <obo:IAO_0000115>An extensive ice shelf fronting the coast of East Antarctica for about 384 km (95E to 105E), projecting seaward about 145 km in the western portion and 64 km in the east.</obo:IAO_0000115>
        <oboInOwl:hasOBONamespace>GAZ</oboInOwl:hasOBONamespace>
        <oboInOwl:id>GAZ:00045074</oboInOwl:id>
        <rdfs:label>Shackleton Ice Shelf</rdfs:label>
    </owl:NamedIndividual>
    


    <!-- http://purl.obolibrary.org/obo/GAZ_00045075 -->

    <owl:NamedIndividual rdf:about="http://purl.obolibrary.org/obo/GAZ_00045075">
        <obo:RO_0001025 rdf:resource="http://purl.obolibrary.org/obo/GAZ_00045074"/>
        <obo:IAO_0000115>An ice-covered island 9 mi long and rising to 240 m, lying 9 mi SE of Masson Island.</obo:IAO_0000115>
        <oboInOwl:hasOBONamespace>GAZ</oboInOwl:hasOBONamespace>
        <oboInOwl:id>GAZ:00045075</oboInOwl:id>
        <rdfs:label>Henderson Island</rdfs:label>
    </owl:NamedIndividual>
    


    <!-- http://purl.obolibrary.org/obo/GAZ_00045076 -->

    <owl:NamedIndividual rdf:about="http://purl.obolibrary.org/obo/GAZ_00045076">
        <obo:RO_0001025 rdf:resource="http://purl.obolibrary.org/obo/GAZ_00004380"/>
        <obo:IAO_0000115>A small rocky island lying 0.4 miles southeast of Norsel Point in Arthur Harbor, off the southwest coast of Anvers Island in the Palmer Archipelago.</obo:IAO_0000115>
        <oboInOwl:hasOBONamespace>GAZ</oboInOwl:hasOBONamespace>
        <oboInOwl:id>GAZ:00045076</oboInOwl:id>
        <rdfs:label>Humble Island</rdfs:label>
    </owl:NamedIndividual>
    


    <!-- http://purl.obolibrary.org/obo/GAZ_00045077 -->

    <owl:NamedIndividual rdf:about="http://purl.obolibrary.org/obo/GAZ_00045077">
        <obo:RO_0001025 rdf:resource="http://purl.obolibrary.org/obo/GAZ_00004045"/>
        <obo:IAO_0000115>A large island off the southeast side and near the northeastern extremity of Antarctic Peninsula, from which it is separated by Prince Gustav Channel.</obo:IAO_0000115>
        <oboInOwl:hasOBONamespace>GAZ</oboInOwl:hasOBONamespace>
        <oboInOwl:id>GAZ:00045077</oboInOwl:id>
        <rdfs:label>James Ross Island</rdfs:label>
    </owl:NamedIndividual>
    


    <!-- http://purl.obolibrary.org/obo/GAZ_00045078 -->

    <owl:NamedIndividual rdf:about="http://purl.obolibrary.org/obo/GAZ_00045078">
        <obo:RO_0001025 rdf:resource="http://purl.obolibrary.org/obo/GAZ_00004380"/>
        <obo:IAO_0000115>A rocky island 0.2 miles long, lying 0.5 miles south of Litchfield Island, off the southwest coast of Anvers Island in the Palmer Archipelago.</obo:IAO_0000115>
        <oboInOwl:hasOBONamespace>GAZ</oboInOwl:hasOBONamespace>
        <oboInOwl:id>GAZ:00045078</oboInOwl:id>
        <rdfs:label>Janus Island</rdfs:label>
    </owl:NamedIndividual>
    


    <!-- http://purl.obolibrary.org/obo/GAZ_00045079 -->

    <owl:NamedIndividual rdf:about="http://purl.obolibrary.org/obo/GAZ_00045079">
        <obo:RO_0001025 rdf:resource="http://purl.obolibrary.org/obo/GAZ_00014089"/>
        <obo:IAO_0000115>A rocky island 2 miles long which rises to 500 m, lying 3 miles east of Cape Alexandra, the southeastern extremity of Adelaide Island, in northern Marguerite Bay.</obo:IAO_0000115>
        <oboInOwl:hasOBONamespace>GAZ</oboInOwl:hasOBONamespace>
        <oboInOwl:id>GAZ:00045079</oboInOwl:id>
        <rdfs:label>Jenny Island</rdfs:label>
    </owl:NamedIndividual>
    


    <!-- http://purl.obolibrary.org/obo/GAZ_00045080 -->

    <owl:NamedIndividual rdf:about="http://purl.obolibrary.org/obo/GAZ_00045080">
        <obo:RO_0001025 rdf:resource="http://purl.obolibrary.org/obo/GAZ_00004380"/>
        <obo:IAO_0000115>A rocky island lying 2 miles southeast of Bonaparte Point, off the southwest coast of Anvers Island in the Palmer Archipelago.</obo:IAO_0000115>
        <oboInOwl:hasOBONamespace>GAZ</oboInOwl:hasOBONamespace>
        <oboInOwl:id>GAZ:00045080</oboInOwl:id>
        <rdfs:label>Laggard Island</rdfs:label>
    </owl:NamedIndividual>
    


    <!-- http://purl.obolibrary.org/obo/GAZ_00045081 -->

    <owl:NamedIndividual rdf:about="http://purl.obolibrary.org/obo/GAZ_00045081">
        <obo:RO_0001025 rdf:resource="http://purl.obolibrary.org/obo/GAZ_00014084"/>
        <obo:IAO_0000115>A low ice-covered island, 35 miles long and more than 10 miles wide, lying 45 miles south of Charcot Island and west of Alexander Island.</obo:IAO_0000115>
        <oboInOwl:hasOBONamespace>GAZ</oboInOwl:hasOBONamespace>
        <oboInOwl:id>GAZ:00045081</oboInOwl:id>
        <rdfs:label>Latady Island</rdfs:label>
    </owl:NamedIndividual>
    


    <!-- http://purl.obolibrary.org/obo/GAZ_00045082 -->

    <owl:NamedIndividual rdf:about="http://purl.obolibrary.org/obo/GAZ_00045082">
        <obo:RO_0001025 rdf:resource="http://purl.obolibrary.org/obo/GAZ_00004380"/>
        <obo:IAO_0000115>An oval-shaped island 0.5 miles long, lying directly east of Christine Island and 1 mile south of Anvers Island.</obo:IAO_0000115>
        <oboInOwl:hasOBONamespace>GAZ</oboInOwl:hasOBONamespace>
        <oboInOwl:id>GAZ:00045082</oboInOwl:id>
        <rdfs:label>Limitrophe Island</rdfs:label>
    </owl:NamedIndividual>
    


    <!-- http://purl.obolibrary.org/obo/GAZ_00045083 -->

    <owl:NamedIndividual rdf:about="http://purl.obolibrary.org/obo/GAZ_00045083">
        <obo:RO_0001025 rdf:resource="http://purl.obolibrary.org/obo/GAZ_00004380"/>
        <obo:IAO_0000115>A small rocky island 0.2 miles west of Litchfield Island, off the southwest coast of Anvers Island, off the Antarctic Peninsula.</obo:IAO_0000115>
        <oboInOwl:hasOBONamespace>GAZ</oboInOwl:hasOBONamespace>
        <oboInOwl:id>GAZ:00045083</oboInOwl:id>
        <rdfs:label>Lipps Island</rdfs:label>
    </owl:NamedIndividual>
    


    <!-- http://purl.obolibrary.org/obo/GAZ_00045084 -->

    <owl:NamedIndividual rdf:about="http://purl.obolibrary.org/obo/GAZ_00045084">
        <obo:RO_0001025 rdf:resource="http://purl.obolibrary.org/obo/GAZ_00139422"/>
        <obo:IAO_0000115>An island about 1.9 km north of Broknes Peninsula in the Larsemann Hills.</obo:IAO_0000115>
        <oboInOwl:hasOBONamespace>GAZ</oboInOwl:hasOBONamespace>
        <oboInOwl:id>GAZ:00045084</oboInOwl:id>
        <rdfs:label>Manning Island</rdfs:label>
    </owl:NamedIndividual>
    


    <!-- http://purl.obolibrary.org/obo/GAZ_00045085 -->

    <owl:NamedIndividual rdf:about="http://purl.obolibrary.org/obo/GAZ_00045085">
        <obo:RO_0001025 rdf:resource="http://purl.obolibrary.org/obo/GAZ_00045074"/>
        <obo:IAO_0000115>An ice-covered island about 17 mi long and rising to 465 m, lying 9 mi NW of Henderson Island within the Shackleton Ice Shelf.</obo:IAO_0000115>
        <oboInOwl:hasOBONamespace>GAZ</oboInOwl:hasOBONamespace>
        <oboInOwl:id>GAZ:00045085</oboInOwl:id>
        <rdfs:label>Masson Island</rdfs:label>
    </owl:NamedIndividual>
    


    <!-- http://purl.obolibrary.org/obo/GAZ_00045086 -->

    <owl:NamedIndividual rdf:about="http://purl.obolibrary.org/obo/GAZ_00045086">
        <obo:RO_0001025 rdf:resource="http://purl.obolibrary.org/obo/GAZ_00045057"/>
        <obo:IAO_0000115>An ice-domed island, 25 miles long and 16 miles wide, lying 25 miles north of the Bunger Hills.</obo:IAO_0000115>
        <oboInOwl:hasOBONamespace>GAZ</oboInOwl:hasOBONamespace>
        <oboInOwl:id>GAZ:00045086</oboInOwl:id>
        <rdfs:label>Mill Island</rdfs:label>
    </owl:NamedIndividual>
    


    <!-- http://purl.obolibrary.org/obo/GAZ_00045087 -->

    <owl:NamedIndividual rdf:about="http://purl.obolibrary.org/obo/GAZ_00045087">
        <obo:RO_0001025 rdf:resource="http://purl.obolibrary.org/obo/GAZ_00141552"/>
        <obo:IAO_0000115>A high rugged island 3 mi in diameter, lying 4 mi S of Cape Calmette, off the W coast of Graham Land.</obo:IAO_0000115>
        <oboInOwl:hasOBONamespace>GAZ</oboInOwl:hasOBONamespace>
        <oboInOwl:id>GAZ:00045087</oboInOwl:id>
        <rdfs:label>Millerand Island</rdfs:label>
    </owl:NamedIndividual>
    


    <!-- http://purl.obolibrary.org/obo/GAZ_00045088 -->

    <owl:NamedIndividual rdf:about="http://purl.obolibrary.org/obo/GAZ_00045088">
        <obo:RO_0001025 rdf:resource="http://purl.obolibrary.org/obo/GAZ_00139422"/>
        <obo:IAO_0000115>A solitary, dark rock, partly ice-covered, 3 mi N of Williams Rocks, off the coast of Mac Robertson Land.</obo:IAO_0000115>
        <oboInOwl:hasOBONamespace>GAZ</oboInOwl:hasOBONamespace>
        <oboInOwl:id>GAZ:00045088</oboInOwl:id>
        <rdfs:label>Nelson Rock</rdfs:label>
    </owl:NamedIndividual>
    


    <!-- http://purl.obolibrary.org/obo/GAZ_00045089 -->

    <owl:NamedIndividual rdf:about="http://purl.obolibrary.org/obo/GAZ_00045089">
        <obo:RO_0001025 rdf:resource="http://purl.obolibrary.org/obo/GAZ_00139422"/>
        <obo:IAO_0000115>A group of rocks 9 mi N of Flat Islands and Holme Bay, off the coast of Mac Robertson Land.</obo:IAO_0000115>
        <oboInOwl:hasOBONamespace>GAZ</oboInOwl:hasOBONamespace>
        <oboInOwl:id>GAZ:00045089</oboInOwl:id>
        <rdfs:label>Williams Rocks</rdfs:label>
    </owl:NamedIndividual>
    


    <!-- http://purl.obolibrary.org/obo/GAZ_00045090 -->

    <owl:NamedIndividual rdf:about="http://purl.obolibrary.org/obo/GAZ_00045090">
        <obo:RO_0001025 rdf:resource="http://purl.obolibrary.org/obo/GAZ_00004380"/>
        <obo:IAO_0000115>An island lying 6 miles west of the north end of Tower Island in the Palmer Archipelago.</obo:IAO_0000115>
        <oboInOwl:hasOBONamespace>GAZ</oboInOwl:hasOBONamespace>
        <oboInOwl:id>GAZ:00045090</oboInOwl:id>
        <rdfs:label>Ohlin Island</rdfs:label>
    </owl:NamedIndividual>
    


    <!-- http://purl.obolibrary.org/obo/GAZ_00045091 -->

    <owl:NamedIndividual rdf:about="http://purl.obolibrary.org/obo/GAZ_00045091">
        <obo:RO_0001025 rdf:resource="http://purl.obolibrary.org/obo/GAZ_00004380"/>
        <obo:IAO_0000115>Two small islands, nearly 0.5 miles apart, and a number of surrounding rocks lying 2 miles southwest of Bonaparte Point, off the southwest coast of Anvers Island in the Palmer Archipelago of Antarctica.</obo:IAO_0000115>
        <oboInOwl:hasOBONamespace>GAZ</oboInOwl:hasOBONamespace>
        <oboInOwl:id>GAZ:00045091</oboInOwl:id>
        <rdfs:label>Outcast Islands</rdfs:label>
    </owl:NamedIndividual>
    


    <!-- http://purl.obolibrary.org/obo/GAZ_00045092 -->

    <owl:NamedIndividual rdf:about="http://purl.obolibrary.org/obo/GAZ_00045092">
        <obo:RO_0001025 rdf:resource="http://purl.obolibrary.org/obo/GAZ_00141552"/>
        <obo:IAO_0000115>A circular volcanic island about 1 mile in diameter, lying 3 miles southeast of Dundee Island, off the northeastern end of the Antarctic Peninsula. The pear-shaped 353 m high island is composed of lava flows capped by a well-preserved cinder cone with a small summit crater. The youthful morphology of the volcano was thought to indicate activity during the last 1000 years (LeMasurier and Thomson 1990). Residual heat keeps the island largely ice free throughout the year.</obo:IAO_0000115>
        <oboInOwl:hasOBONamespace>GAZ</oboInOwl:hasOBONamespace>
        <oboInOwl:id>GAZ:00045092</oboInOwl:id>
        <rdfs:label>Paulet Island</rdfs:label>
    </owl:NamedIndividual>
    


    <!-- http://purl.obolibrary.org/obo/GAZ_00045093 -->

    <owl:NamedIndividual rdf:about="http://purl.obolibrary.org/obo/GAZ_00045093">
        <obo:RO_0001025 rdf:resource="http://purl.obolibrary.org/obo/GAZ_00023304"/>
        <obo:IAO_0000115>A group of small islands and rocks extending over an area of about 7 miles, lying in the western part of the Ross Sea, 5 miles southeast of Cape McCormick, Victoria Land.</obo:IAO_0000115>
        <oboInOwl:hasOBONamespace>GAZ</oboInOwl:hasOBONamespace>
        <oboInOwl:id>GAZ:00045093</oboInOwl:id>
        <rdfs:label>Possession Islands</rdfs:label>
    </owl:NamedIndividual>
    


    <!-- http://purl.obolibrary.org/obo/GAZ_00045094 -->

    <owl:NamedIndividual rdf:about="http://purl.obolibrary.org/obo/GAZ_00045094">
        <obo:RO_0001025 rdf:resource="http://purl.obolibrary.org/obo/GAZ_00045093"/>
        <obo:IAO_0000115>A rocky island nearly 2 miles long, which is the northernmost and largest of the Possession Islands.</obo:IAO_0000115>
        <oboInOwl:hasOBONamespace>GAZ</oboInOwl:hasOBONamespace>
        <oboInOwl:id>GAZ:00045094</oboInOwl:id>
        <rdfs:label>Possession Island</rdfs:label>
    </owl:NamedIndividual>
    


    <!-- http://purl.obolibrary.org/obo/GAZ_00045095 -->

    <owl:NamedIndividual rdf:about="http://purl.obolibrary.org/obo/GAZ_00045095">
        <obo:RO_0001025 rdf:resource="http://purl.obolibrary.org/obo/GAZ_00004045"/>
        <obo:IAO_0000115>An ice-covered island, 13 miles long in a northwest-southeast direction and 6 miles wide, lying at the east end of the Seal Nunataks off the east coast of the Antarctic Peninsula.</obo:IAO_0000115>
        <oboInOwl:hasOBONamespace>GAZ</oboInOwl:hasOBONamespace>
        <oboInOwl:id>GAZ:00045095</oboInOwl:id>
        <rdfs:label>Robertson Island</rdfs:label>
    </owl:NamedIndividual>
    


    <!-- http://purl.obolibrary.org/obo/GAZ_00045096 -->

    <owl:NamedIndividual rdf:about="http://purl.obolibrary.org/obo/GAZ_00045096">
        <obo:RO_0001025 rdf:resource="http://purl.obolibrary.org/obo/GAZ_00023304"/>
        <obo:IAO_0000115>An ice-covered island, about 130 km long in a NW-SE direction, 65 km wide and about 7,500 km2 in area, lying in the E part of the Ross Ice Shelf of Antarctica. Its central ridge rises to about 550 m above sea level.</obo:IAO_0000115>
        <oboInOwl:hasOBONamespace>GAZ</oboInOwl:hasOBONamespace>
        <oboInOwl:id>GAZ:00045096</oboInOwl:id>
        <rdfs:label>Roosevelt Island</rdfs:label>
    </owl:NamedIndividual>
    


    <!-- http://purl.obolibrary.org/obo/GAZ_00045097 -->

    <owl:NamedIndividual rdf:about="http://purl.obolibrary.org/obo/GAZ_00045097">
        <obo:RO_0001025 rdf:resource="http://purl.obolibrary.org/obo/GAZ_00023304"/>
        <obo:IAO_0000115>An island, 0.25 mi long and half as wide, lying 315 mi northeastward of Cape Adare, the northeastern extremity of Victoria Land.</obo:IAO_0000115>
        <oboInOwl:hasOBONamespace>GAZ</oboInOwl:hasOBONamespace>
        <oboInOwl:id>GAZ:00045097</oboInOwl:id>
        <rdfs:label>Scott Island</rdfs:label>
    </owl:NamedIndividual>
    


    <!-- http://purl.obolibrary.org/obo/GAZ_00045098 -->

    <owl:NamedIndividual rdf:about="http://purl.obolibrary.org/obo/GAZ_00045098">
        <obo:RO_0001025 rdf:resource="http://purl.obolibrary.org/obo/GAZ_00023304"/>
        <obo:IAO_0000115>A stack to the W of Scott Island, reaching over 60m.</obo:IAO_0000115>
        <oboInOwl:hasOBONamespace>GAZ</oboInOwl:hasOBONamespace>
        <oboInOwl:id>GAZ:00045098</oboInOwl:id>
        <rdfs:label>Haggitt&apos;s Pillar</rdfs:label>
    </owl:NamedIndividual>
    


    <!-- http://purl.obolibrary.org/obo/GAZ_00045099 -->

    <owl:NamedIndividual rdf:about="http://purl.obolibrary.org/obo/GAZ_00045099">
        <obo:RO_0001025 rdf:resource="http://purl.obolibrary.org/obo/GAZ_00014084"/>
        <obo:IAO_0000115>A large ice-covered island of Antarctica. It lies south west of Alexander Island and west of the base of the Antarctic Peninsula, close to the coast of Ellsworth Land, 30 miles east of Smyley Island. It is 50 miles long and 25 miles wide.</obo:IAO_0000115>
        <oboInOwl:hasOBONamespace>GAZ</oboInOwl:hasOBONamespace>
        <oboInOwl:id>GAZ:00045099</oboInOwl:id>
        <rdfs:label>Spaatz Island</rdfs:label>
    </owl:NamedIndividual>
    


    <!-- http://purl.obolibrary.org/obo/GAZ_00045100 -->

    <owl:NamedIndividual rdf:about="http://purl.obolibrary.org/obo/GAZ_00045100">
        <obo:RO_0001025 rdf:resource="http://purl.obolibrary.org/obo/GAZ_00014084"/>
        <obo:IAO_0000115>An Antarctic island lying off the Antarctic Peninsula.</obo:IAO_0000115>
        <oboInOwl:hasOBONamespace>GAZ</oboInOwl:hasOBONamespace>
        <oboInOwl:id>GAZ:00045100</oboInOwl:id>
        <rdfs:label>Smyley Island</rdfs:label>
    </owl:NamedIndividual>
    


    <!-- http://purl.obolibrary.org/obo/GAZ_00045101 -->

    <owl:NamedIndividual rdf:about="http://purl.obolibrary.org/obo/GAZ_00045101">
        <obo:RO_0001025 rdf:resource="http://purl.obolibrary.org/obo/GAZ_00004380"/>
        <obo:IAO_0000115>A distinctive oval-shaped rock, cleanly split in a north-south direction to the water line, lying 0.1 mi NW of Janus Island, off the SW coast of Anvers Island.</obo:IAO_0000115>
        <oboInOwl:hasOBONamespace>GAZ</oboInOwl:hasOBONamespace>
        <oboInOwl:id>GAZ:00045101</oboInOwl:id>
        <rdfs:label>Split Rock</rdfs:label>
    </owl:NamedIndividual>
    


    <!-- http://purl.obolibrary.org/obo/GAZ_00045102 -->

    <owl:NamedIndividual rdf:about="http://purl.obolibrary.org/obo/GAZ_00045102">
        <obo:RO_0001025 rdf:resource="http://purl.obolibrary.org/obo/GAZ_00004380"/>
        <obo:IAO_0000115>A small, low, rocky island lying 1.5 miles southwest of Bonaparte Point, off the southwest coast of Anvers Island in the Palmer Archipelago.</obo:IAO_0000115>
        <oboInOwl:hasOBONamespace>GAZ</oboInOwl:hasOBONamespace>
        <oboInOwl:id>GAZ:00045102</oboInOwl:id>
        <rdfs:label>Spume Island</rdfs:label>
    </owl:NamedIndividual>
    


    <!-- http://purl.obolibrary.org/obo/GAZ_00045103 -->

    <owl:NamedIndividual rdf:about="http://purl.obolibrary.org/obo/GAZ_00045103">
        <obo:RO_0001025 rdf:resource="http://purl.obolibrary.org/obo/GAZ_00004380"/>
        <obo:IAO_0000115>Three prominent rocks lying 0.5 miles north of Limitrophe Island, off the southwest coast of Anvers Island.</obo:IAO_0000115>
        <oboInOwl:hasOBONamespace>GAZ</oboInOwl:hasOBONamespace>
        <oboInOwl:id>GAZ:00045103</oboInOwl:id>
        <rdfs:label>Stepping Stones</rdfs:label>
    </owl:NamedIndividual>
    


    <!-- http://purl.obolibrary.org/obo/GAZ_00045104 -->

    <owl:NamedIndividual rdf:about="http://purl.obolibrary.org/obo/GAZ_00045104">
        <obo:RO_0001025 rdf:resource="http://purl.obolibrary.org/obo/GAZ_00004380"/>
        <obo:IAO_0000115>A sub-antarctic island 8 km long and 305 m high, lying 32 km northeast of Trinity Island and marking the northeast extent of Palmer Archipelago.</obo:IAO_0000115>
        <oboInOwl:hasOBONamespace>GAZ</oboInOwl:hasOBONamespace>
        <oboInOwl:id>GAZ:00045104</oboInOwl:id>
        <rdfs:label>Tower Island</rdfs:label>
    </owl:NamedIndividual>
    


    <!-- http://purl.obolibrary.org/obo/GAZ_00045105 -->

    <owl:NamedIndividual rdf:about="http://purl.obolibrary.org/obo/GAZ_00045105">
        <obo:RO_0001025 rdf:resource="http://purl.obolibrary.org/obo/GAZ_00004380"/>
        <obo:IAO_0000115>An island 15 miles long and 6 miles wide in the northern part of the Palmer Archipelago.</obo:IAO_0000115>
        <oboInOwl:hasOBONamespace>GAZ</oboInOwl:hasOBONamespace>
        <oboInOwl:id>GAZ:00045105</oboInOwl:id>
        <rdfs:label>Trinity Island</rdfs:label>
    </owl:NamedIndividual>
    


    <!-- http://purl.obolibrary.org/obo/GAZ_00045106 -->

    <owl:NamedIndividual rdf:about="http://purl.obolibrary.org/obo/GAZ_00045106">
        <obo:RO_0001025 rdf:resource="http://purl.obolibrary.org/obo/GAZ_00004045"/>
        <obo:IAO_0000115>A small island to the northwest of James Ross Island, on the Antarctic Peninsula.</obo:IAO_0000115>
        <oboInOwl:hasOBONamespace>GAZ</oboInOwl:hasOBONamespace>
        <oboInOwl:id>GAZ:00045106</oboInOwl:id>
        <rdfs:label>Vega Island</rdfs:label>
    </owl:NamedIndividual>
    


    <!-- http://purl.obolibrary.org/obo/GAZ_00045107 -->

    <owl:NamedIndividual rdf:about="http://purl.obolibrary.org/obo/GAZ_00045107">
        <obo:RO_0001025 rdf:resource="http://purl.obolibrary.org/obo/GAZ_00014094"/>
        <obo:IAO_0000115>A rocky, triangular-shaped Antarctic island, 1.7 mi long, marking the southwest end of the Windmill Islands.</obo:IAO_0000115>
        <oboInOwl:hasOBONamespace>GAZ</oboInOwl:hasOBONamespace>
        <oboInOwl:id>GAZ:00045107</oboInOwl:id>
        <rdfs:label>Holl Island</rdfs:label>
    </owl:NamedIndividual>
    


    <!-- http://purl.obolibrary.org/obo/GAZ_00045108 -->

    <owl:NamedIndividual rdf:about="http://purl.obolibrary.org/obo/GAZ_00045108">
        <obo:RO_0001025 rdf:resource="http://purl.obolibrary.org/obo/GAZ_00014094"/>
        <obo:IAO_0000115>Two Antarctic islands lying close to Tracy Point, the western extremity of Beall Island, in the Windmill Islands.</obo:IAO_0000115>
        <oboInOwl:hasOBONamespace>GAZ</oboInOwl:hasOBONamespace>
        <oboInOwl:id>GAZ:00045108</oboInOwl:id>
        <rdfs:label>Smith Islands</rdfs:label>
    </owl:NamedIndividual>
    


    <!-- http://purl.obolibrary.org/obo/GAZ_00045109 -->

    <owl:NamedIndividual rdf:about="http://purl.obolibrary.org/obo/GAZ_00045109">
        <obo:RO_0001025 rdf:resource="http://purl.obolibrary.org/obo/GAZ_00014094"/>
        <obo:IAO_0000115>A small, mainly ice-covered Antarctic island lying between Robinson Ridge and Odbert Island, in the Windmill Islands.</obo:IAO_0000115>
        <oboInOwl:hasOBONamespace>GAZ</oboInOwl:hasOBONamespace>
        <oboInOwl:id>GAZ:00045109</oboInOwl:id>
        <rdfs:label>Hemphill Island</rdfs:label>
    </owl:NamedIndividual>
    


    <!-- http://purl.obolibrary.org/obo/GAZ_00045110 -->

    <owl:NamedIndividual rdf:about="http://purl.obolibrary.org/obo/GAZ_00045110">
        <obo:RO_0001025 rdf:resource="http://purl.obolibrary.org/obo/GAZ_00014094"/>
        <obo:IAO_0000115>An exposed reef lying half a mile west of Clark Peninsula, in the Windmill Islands, Antarctica.</obo:IAO_0000115>
        <oboInOwl:hasOBONamespace>GAZ</oboInOwl:hasOBONamespace>
        <oboInOwl:id>GAZ:00045110</oboInOwl:id>
        <rdfs:label>Gibney Reef</rdfs:label>
    </owl:NamedIndividual>
    


    <!-- http://purl.obolibrary.org/obo/GAZ_00045111 -->

    <owl:NamedIndividual rdf:about="http://purl.obolibrary.org/obo/GAZ_00045111">
        <obo:RO_0001025 rdf:resource="http://purl.obolibrary.org/obo/GAZ_00014094"/>
        <obo:IAO_0000115>A rocky Antarctic island a mile long, lying 0.1 mi northwest of the western end of Bailey Peninsula, in the Windmill Islands.</obo:IAO_0000115>
        <oboInOwl:hasOBONamespace>GAZ</oboInOwl:hasOBONamespace>
        <oboInOwl:id>GAZ:00045111</oboInOwl:id>
        <rdfs:label>Shirley Island</rdfs:label>
    </owl:NamedIndividual>
    


    <!-- http://purl.obolibrary.org/obo/GAZ_00045112 -->

    <owl:NamedIndividual rdf:about="http://purl.obolibrary.org/obo/GAZ_00045112">
        <obo:RO_0001025 rdf:resource="http://purl.obolibrary.org/obo/GAZ_00014094"/>
        <obo:IAO_0000115>A rocky Antarctic island, 2 km long, between O&apos;Connor and Cloyd Islands in the southern part of the Windmill Islands.</obo:IAO_0000115>
        <oboInOwl:hasOBONamespace>GAZ</oboInOwl:hasOBONamespace>
        <oboInOwl:id>GAZ:00045112</oboInOwl:id>
        <rdfs:label>Ford Island</rdfs:label>
    </owl:NamedIndividual>
    


    <!-- http://purl.obolibrary.org/obo/GAZ_00045113 -->

    <owl:NamedIndividual rdf:about="http://purl.obolibrary.org/obo/GAZ_00045113">
        <obo:RO_0001025 rdf:resource="http://purl.obolibrary.org/obo/GAZ_00014094"/>
        <obo:IAO_0000115>An Antarctic rocky island, 2 mi long, with two inlets indenting the north side, lying immediately west of Browning Peninsula in the south part of the Windmill Islands.</obo:IAO_0000115>
        <oboInOwl:hasOBONamespace>GAZ</oboInOwl:hasOBONamespace>
        <oboInOwl:id>GAZ:00045113</oboInOwl:id>
        <rdfs:label>Peterson Island</rdfs:label>
    </owl:NamedIndividual>
    


    <!-- http://purl.obolibrary.org/obo/GAZ_00045114 -->

    <owl:NamedIndividual rdf:about="http://purl.obolibrary.org/obo/GAZ_00045114">
        <obo:RO_0001025 rdf:resource="http://purl.obolibrary.org/obo/GAZ_00014094"/>
        <obo:IAO_0000115>An Antarctic rocky island, 2 mi long, lying one mile east of Cloyd Island in the south part of the Windmill Islands.</obo:IAO_0000115>
        <oboInOwl:hasOBONamespace>GAZ</oboInOwl:hasOBONamespace>
        <oboInOwl:id>GAZ:00045114</oboInOwl:id>
        <rdfs:label>Herring Island</rdfs:label>
    </owl:NamedIndividual>
    


    <!-- http://purl.obolibrary.org/obo/GAZ_00045115 -->

    <owl:NamedIndividual rdf:about="http://purl.obolibrary.org/obo/GAZ_00045115">
        <obo:RO_0001025 rdf:resource="http://purl.obolibrary.org/obo/GAZ_00014094"/>
        <obo:IAO_0000115>An Antarctic island about a mile long, lying north of Midgley Island, in the Windmill Islands.</obo:IAO_0000115>
        <oboInOwl:hasOBONamespace>GAZ</oboInOwl:hasOBONamespace>
        <oboInOwl:id>GAZ:00045115</oboInOwl:id>
        <rdfs:label>Hollin Island</rdfs:label>
    </owl:NamedIndividual>
    


    <!-- http://purl.obolibrary.org/obo/GAZ_00045116 -->

    <owl:NamedIndividual rdf:about="http://purl.obolibrary.org/obo/GAZ_00045116">
        <obo:RO_0001025 rdf:resource="http://purl.obolibrary.org/obo/GAZ_00014094"/>
        <obo:IAO_0000115>A low ice-capped rock lying half a mile northwest of Kilby Island at the mouth of Newcomb Bay, in the Windmill Islands, Antarctica.</obo:IAO_0000115>
        <oboInOwl:hasOBONamespace>GAZ</oboInOwl:hasOBONamespace>
        <oboInOwl:id>GAZ:00045116</oboInOwl:id>
        <rdfs:label>Fitzpatrick Rock</rdfs:label>
    </owl:NamedIndividual>
    


    <!-- http://purl.obolibrary.org/obo/GAZ_00045117 -->

    <owl:NamedIndividual rdf:about="http://purl.obolibrary.org/obo/GAZ_00045117">
        <obo:RO_0001025 rdf:resource="http://purl.obolibrary.org/obo/GAZ_00014094"/>
        <obo:IAO_0000115>A rocky Antarctic island, a mile long, between Midgley Island and Mitchell Peninsula in the Windmill Islands.</obo:IAO_0000115>
        <oboInOwl:hasOBONamespace>GAZ</oboInOwl:hasOBONamespace>
        <oboInOwl:id>GAZ:00045117</oboInOwl:id>
        <rdfs:label>Pidgeon Island</rdfs:label>
    </owl:NamedIndividual>
    


    <!-- http://purl.obolibrary.org/obo/GAZ_00045118 -->

    <owl:NamedIndividual rdf:about="http://purl.obolibrary.org/obo/GAZ_00045118">
        <obo:RO_0001025 rdf:resource="http://purl.obolibrary.org/obo/GAZ_00014094"/>
        <obo:IAO_0000115>A small Antarctic island at the south entrance to Robertson Channel in the Windmill Islands.</obo:IAO_0000115>
        <oboInOwl:hasOBONamespace>GAZ</oboInOwl:hasOBONamespace>
        <oboInOwl:id>GAZ:00045118</oboInOwl:id>
        <rdfs:label>Griffith Island</rdfs:label>
    </owl:NamedIndividual>
    


    <!-- http://purl.obolibrary.org/obo/GAZ_00045119 -->

    <owl:NamedIndividual rdf:about="http://purl.obolibrary.org/obo/GAZ_00045119">
        <obo:RO_0001025 rdf:resource="http://purl.obolibrary.org/obo/GAZ_00014094"/>
        <obo:IAO_0000115>A rocky Antarctic island, 0.2 mi long, lying northeast of McMullin Island in the entrance of Newcomb Bay, in the Windmill Islands.</obo:IAO_0000115>
        <oboInOwl:hasOBONamespace>GAZ</oboInOwl:hasOBONamespace>
        <oboInOwl:id>GAZ:00045119</oboInOwl:id>
        <rdfs:label>Kilby Island</rdfs:label>
    </owl:NamedIndividual>
    


    <!-- http://purl.obolibrary.org/obo/GAZ_00045120 -->

    <owl:NamedIndividual rdf:about="http://purl.obolibrary.org/obo/GAZ_00045120">
        <obo:RO_0001025 rdf:resource="http://purl.obolibrary.org/obo/GAZ_00014094"/>
        <obo:IAO_0000115>A small Antarctic island just west of Blakeney Point, Clark Peninsula, in the Windmill Islands.</obo:IAO_0000115>
        <oboInOwl:hasOBONamespace>GAZ</oboInOwl:hasOBONamespace>
        <oboInOwl:id>GAZ:00045120</oboInOwl:id>
        <rdfs:label>McIntyre Island</rdfs:label>
    </owl:NamedIndividual>
    


    <!-- http://purl.obolibrary.org/obo/GAZ_00045121 -->

    <owl:NamedIndividual rdf:about="http://purl.obolibrary.org/obo/GAZ_00045121">
        <obo:RO_0001025 rdf:resource="http://purl.obolibrary.org/obo/GAZ_00014094"/>
        <obo:IAO_0000115>A steep, rocky island, 0.6 mi long, lying 1.1 mi west of Odbert Island in the Windmill Islands.</obo:IAO_0000115>
        <oboInOwl:hasOBONamespace>GAZ</oboInOwl:hasOBONamespace>
        <oboInOwl:id>GAZ:00045121</oboInOwl:id>
        <rdfs:label>Ardery Island</rdfs:label>
    </owl:NamedIndividual>
    


    <!-- http://purl.obolibrary.org/obo/GAZ_00045122 -->

    <owl:NamedIndividual rdf:about="http://purl.obolibrary.org/obo/GAZ_00045122">
        <obo:RO_0001025 rdf:resource="http://purl.obolibrary.org/obo/GAZ_00014094"/>
        <obo:IAO_0000115>A group of islands lying northeast of Hollin Island, in the Windmill Islands.</obo:IAO_0000115>
        <oboInOwl:hasOBONamespace>GAZ</oboInOwl:hasOBONamespace>
        <oboInOwl:id>GAZ:00045122</oboInOwl:id>
        <rdfs:label>Cronk Islands</rdfs:label>
    </owl:NamedIndividual>
    


    <!-- http://purl.obolibrary.org/obo/GAZ_00045123 -->

    <owl:NamedIndividual rdf:about="http://purl.obolibrary.org/obo/GAZ_00045123">
        <obo:RO_0001025 rdf:resource="http://purl.obolibrary.org/obo/GAZ_00014094"/>
        <obo:IAO_0000115>A small Antarctic island in the extreme southern lobe of Penney Bay, in the Windmill Islands.</obo:IAO_0000115>
        <oboInOwl:hasOBONamespace>GAZ</oboInOwl:hasOBONamespace>
        <oboInOwl:id>GAZ:00045123</oboInOwl:id>
        <rdfs:label>Austral Island</rdfs:label>
    </owl:NamedIndividual>
    


    <!-- http://purl.obolibrary.org/obo/GAZ_00045124 -->

    <owl:NamedIndividual rdf:about="http://purl.obolibrary.org/obo/GAZ_00045124">
        <obo:RO_0001025 rdf:resource="http://purl.obolibrary.org/obo/GAZ_00014094"/>
        <obo:IAO_0000115>A small Antarctic island lying off the western side of Hollin Island, in the Windmill Islands.</obo:IAO_0000115>
        <oboInOwl:hasOBONamespace>GAZ</oboInOwl:hasOBONamespace>
        <oboInOwl:id>GAZ:00045124</oboInOwl:id>
        <rdfs:label>Borrello Island</rdfs:label>
    </owl:NamedIndividual>
    


    <!-- http://purl.obolibrary.org/obo/GAZ_00045125 -->

    <owl:NamedIndividual rdf:about="http://purl.obolibrary.org/obo/GAZ_00045125">
        <obo:RO_0001025 rdf:resource="http://purl.obolibrary.org/obo/GAZ_00014094"/>
        <obo:IAO_0000115>A small chain of rocks in the Antarctic Windmill Islands which extends northeast from the north side of Bailey Peninsula into Newcomb Bay.</obo:IAO_0000115>
        <oboInOwl:hasOBONamespace>GAZ</oboInOwl:hasOBONamespace>
        <oboInOwl:id>GAZ:00045125</oboInOwl:id>
        <rdfs:label>Bailey Rocks</rdfs:label>
    </owl:NamedIndividual>
    


    <!-- http://purl.obolibrary.org/obo/GAZ_00045126 -->

    <owl:NamedIndividual rdf:about="http://purl.obolibrary.org/obo/GAZ_00045126">
        <obo:RO_0001025 rdf:resource="http://purl.obolibrary.org/obo/GAZ_00014094"/>
        <obo:IAO_0000115>A mainly ice-free Antarctic island lying south of Boffa Island in the Windmill Islands.</obo:IAO_0000115>
        <oboInOwl:hasOBONamespace>GAZ</oboInOwl:hasOBONamespace>
        <oboInOwl:id>GAZ:00045126</oboInOwl:id>
        <rdfs:label>Birkenhauer Island</rdfs:label>
    </owl:NamedIndividual>
    


    <!-- http://purl.obolibrary.org/obo/GAZ_00045127 -->

    <owl:NamedIndividual rdf:about="http://purl.obolibrary.org/obo/GAZ_00045127">
        <obo:RO_0001025 rdf:resource="http://purl.obolibrary.org/obo/GAZ_00014094"/>
        <obo:IAO_0000115>An Antarctic rocky island, 0.3 mi long, lying 0.1 mi northwest of Boffa Island and half a mile east of Browning Peninsula in the south part of the Windmill Islands.</obo:IAO_0000115>
        <oboInOwl:hasOBONamespace>GAZ</oboInOwl:hasOBONamespace>
        <oboInOwl:id>GAZ:00045127</oboInOwl:id>
        <rdfs:label>Bosner Island</rdfs:label>
    </owl:NamedIndividual>
    


    <!-- http://purl.obolibrary.org/obo/GAZ_00045128 -->

    <owl:NamedIndividual rdf:about="http://purl.obolibrary.org/obo/GAZ_00045128">
        <obo:RO_0001025 rdf:resource="http://purl.obolibrary.org/obo/GAZ_00014094"/>
        <obo:IAO_0000115>An Antarctic rocky island, 1.1 mi long, with small coves indenting the east and west sides, lying 0.2 mi northwest of Mitchell Peninsula in the Windmill Islands.</obo:IAO_0000115>
        <oboInOwl:hasOBONamespace>GAZ</oboInOwl:hasOBONamespace>
        <oboInOwl:id>GAZ:00045128</oboInOwl:id>
        <rdfs:label>Beall Island</rdfs:label>
    </owl:NamedIndividual>
    


    <!-- http://purl.obolibrary.org/obo/GAZ_00045129 -->

    <owl:NamedIndividual rdf:about="http://purl.obolibrary.org/obo/GAZ_00045129">
        <obo:RO_0001025 rdf:resource="http://purl.obolibrary.org/obo/GAZ_00014094"/>
        <obo:IAO_0000115>A rocky Antarctic island, 0.6 mi long, between Ford and Herring Islands in the south part of the Windmill Islands.</obo:IAO_0000115>
        <oboInOwl:hasOBONamespace>GAZ</oboInOwl:hasOBONamespace>
        <oboInOwl:id>GAZ:00045129</oboInOwl:id>
        <rdfs:label>Cloyd Island</rdfs:label>
    </owl:NamedIndividual>
    


    <!-- http://purl.obolibrary.org/obo/GAZ_00045130 -->

    <owl:NamedIndividual rdf:about="http://purl.obolibrary.org/obo/GAZ_00045130">
        <obo:RO_0001025 rdf:resource="http://purl.obolibrary.org/obo/GAZ_00014094"/>
        <obo:IAO_0000115>An island 0.3 mi long, that lies immediately east of Herring Island in the Windmill Islands.</obo:IAO_0000115>
        <oboInOwl:hasOBONamespace>GAZ</oboInOwl:hasOBONamespace>
        <oboInOwl:id>GAZ:00045130</oboInOwl:id>
        <rdfs:label>Bousquet Island</rdfs:label>
    </owl:NamedIndividual>
    


    <!-- http://purl.obolibrary.org/obo/GAZ_00045131 -->

    <owl:NamedIndividual rdf:about="http://purl.obolibrary.org/obo/GAZ_00045131">
        <obo:RO_0001025 rdf:resource="http://purl.obolibrary.org/obo/GAZ_00014094"/>
        <obo:IAO_0000115>A rocky, ridge-like Antarctic island, 0.8 mi long, lying half a mile east of Browning Peninsula between Bosner and Birkenhauer Islands, in the south part of the Windmill Islands.</obo:IAO_0000115>
        <oboInOwl:hasOBONamespace>GAZ</oboInOwl:hasOBONamespace>
        <oboInOwl:id>GAZ:00045131</oboInOwl:id>
        <rdfs:label>Boffa Island</rdfs:label>
    </owl:NamedIndividual>
    


    <!-- http://purl.obolibrary.org/obo/GAZ_00045132 -->

    <owl:NamedIndividual rdf:about="http://purl.obolibrary.org/obo/GAZ_00045132">
        <obo:RO_0001025 rdf:resource="http://purl.obolibrary.org/obo/GAZ_00014094"/>
        <obo:IAO_0000115>A small Antarctic island in the south part of Newcomb Bay, lying 0.1 mi east of McMullin Island in the Windmill Islands.</obo:IAO_0000115>
        <oboInOwl:hasOBONamespace>GAZ</oboInOwl:hasOBONamespace>
        <oboInOwl:id>GAZ:00045132</oboInOwl:id>
        <rdfs:label>Boving Island</rdfs:label>
    </owl:NamedIndividual>
    


    <!-- http://purl.obolibrary.org/obo/GAZ_00045133 -->

    <owl:NamedIndividual rdf:about="http://purl.obolibrary.org/obo/GAZ_00045133">
        <obo:RO_0001025 rdf:resource="http://purl.obolibrary.org/obo/GAZ_00014094"/>
        <obo:IAO_0000115>An Antarctic island lying a quarter mile west of Beall Island in the Windmill Islands.</obo:IAO_0000115>
        <oboInOwl:hasOBONamespace>GAZ</oboInOwl:hasOBONamespace>
        <oboInOwl:id>GAZ:00045133</oboInOwl:id>
        <rdfs:label>Denison Island</rdfs:label>
    </owl:NamedIndividual>
    


    <!-- http://purl.obolibrary.org/obo/GAZ_00045134 -->

    <owl:NamedIndividual rdf:about="http://purl.obolibrary.org/obo/GAZ_00045134">
        <obo:RO_0001025 rdf:resource="http://purl.obolibrary.org/obo/GAZ_00014094"/>
        <obo:IAO_0000115>A small chain of Antarctic islands lying in the north side of the entrance to Sparkes Bay in the Windmill Islands.</obo:IAO_0000115>
        <oboInOwl:hasOBONamespace>GAZ</oboInOwl:hasOBONamespace>
        <oboInOwl:id>GAZ:00045134</oboInOwl:id>
        <rdfs:label>Allison Islands</rdfs:label>
    </owl:NamedIndividual>
    


    <!-- http://purl.obolibrary.org/obo/GAZ_00048397 -->

    <owl:NamedIndividual rdf:about="http://purl.obolibrary.org/obo/GAZ_00048397">
        <obo:RO_0001025 rdf:resource="http://purl.obolibrary.org/obo/GAZ_00023325"/>
        <obo:IAO_0000115>The largest of the Larsen Islands, lying off the W end of Coronation Island in the South Orkney Islands.</obo:IAO_0000115>
        <oboInOwl:hasOBONamespace>GAZ</oboInOwl:hasOBONamespace>
        <oboInOwl:id>GAZ:00048397</oboInOwl:id>
        <rdfs:label>Monroe Island</rdfs:label>
    </owl:NamedIndividual>
    


    <!-- http://purl.obolibrary.org/obo/GAZ_00048398 -->

    <owl:NamedIndividual rdf:about="http://purl.obolibrary.org/obo/GAZ_00048398">
        <obo:RO_0001025 rdf:resource="http://purl.obolibrary.org/obo/GAZ_00009523"/>
        <obo:IAO_0000115>An island lying in the E part of Marshall Bay, close off the S coast of Coronation Island in the South Orkney Islands.</obo:IAO_0000115>
        <oboInOwl:hasOBONamespace>GAZ</oboInOwl:hasOBONamespace>
        <oboInOwl:id>GAZ:00048398</oboInOwl:id>
        <rdfs:label>Lynch Island</rdfs:label>
    </owl:NamedIndividual>
    


    <!-- http://purl.obolibrary.org/obo/GAZ_00048399 -->

    <owl:NamedIndividual rdf:about="http://purl.obolibrary.org/obo/GAZ_00048399">
        <obo:RO_0001025 rdf:resource="http://purl.obolibrary.org/obo/GAZ_00014085"/>
        <obo:IAO_0000115>An ice-covered island, 20 mi long and 10 mi wide, lying within the Getz Ice Shelf and midway between Grant Island and Siple Island, off the coast of Marie Byrd Land.</obo:IAO_0000115>
        <oboInOwl:hasOBONamespace>GAZ</oboInOwl:hasOBONamespace>
        <oboInOwl:id>GAZ:00048399</oboInOwl:id>
        <rdfs:label>Dean Island</rdfs:label>
    </owl:NamedIndividual>
    


    <!-- http://purl.obolibrary.org/obo/GAZ_00048400 -->

    <owl:NamedIndividual rdf:about="http://purl.obolibrary.org/obo/GAZ_00048400">
        <obo:RO_0001025 rdf:resource="http://purl.obolibrary.org/obo/GAZ_00051503"/>
        <obo:RO_0001025 rdf:resource="http://purl.obolibrary.org/obo/GAZ_00051504"/>
        <obo:IAO_0000115>An ice-covered island of Antarctica about 51 km long and 16 km wide, lying south of Thurston Island in the middle of Peacock Sound. The feature rises above the Abbot Ice Shelf which occupies the sound.</obo:IAO_0000115>
        <oboInOwl:hasOBONamespace>GAZ</oboInOwl:hasOBONamespace>
        <oboInOwl:id>GAZ:00048400</oboInOwl:id>
        <rdfs:label>Sherman Island</rdfs:label>
    </owl:NamedIndividual>
    


    <!-- http://purl.obolibrary.org/obo/GAZ_00048401 -->

    <owl:NamedIndividual rdf:about="http://purl.obolibrary.org/obo/GAZ_00048401">
        <obo:RO_0001025 rdf:resource="http://purl.obolibrary.org/obo/GAZ_00004045"/>
        <obo:IAO_0000115>Rounded, ice-covered island, 13 mi long, lying 8 mi E of Cape Boggs, off the E coast of Palmer Land.</obo:IAO_0000115>
        <oboInOwl:hasOBONamespace>GAZ</oboInOwl:hasOBONamespace>
        <oboInOwl:id>GAZ:00048401</oboInOwl:id>
        <rdfs:label>Dolleman Island</rdfs:label>
    </owl:NamedIndividual>
    


    <!-- http://purl.obolibrary.org/obo/GAZ_00048402 -->

    <owl:NamedIndividual rdf:about="http://purl.obolibrary.org/obo/GAZ_00048402">
        <obo:RO_0001025 rdf:resource="http://purl.obolibrary.org/obo/GAZ_00014085"/>
        <obo:RO_0001025 rdf:resource="http://purl.obolibrary.org/obo/GAZ_00051504"/>
        <obo:IAO_0000115>An island about 29 km long, lying 24 km southeast of Cape Annawan, Thurston Island. The feature forms the SE limit of Seraph Bay.</obo:IAO_0000115>
        <oboInOwl:hasOBONamespace>GAZ</oboInOwl:hasOBONamespace>
        <oboInOwl:id>GAZ:00048402</oboInOwl:id>
        <rdfs:label>Dustin Island</rdfs:label>
    </owl:NamedIndividual>
    


    <!-- http://purl.obolibrary.org/obo/GAZ_00048403 -->

    <owl:NamedIndividual rdf:about="http://purl.obolibrary.org/obo/GAZ_00048403">
        <obo:RO_0001025 rdf:resource="http://purl.obolibrary.org/obo/GAZ_00004045"/>
        <obo:IAO_0000115>An ice-covered, dome-shaped island 8 miles in diameter, lying 15 miles northeast of Cape Collier, off the east coast of Palmer Land.</obo:IAO_0000115>
        <oboInOwl:hasOBONamespace>GAZ</oboInOwl:hasOBONamespace>
        <oboInOwl:id>GAZ:00048403</oboInOwl:id>
        <rdfs:label>Ewing Island</rdfs:label>
    </owl:NamedIndividual>
    


    <!-- http://purl.obolibrary.org/obo/GAZ_00048404 -->

    <owl:NamedIndividual rdf:about="http://purl.obolibrary.org/obo/GAZ_00048404">
        <obo:RO_0001025 rdf:resource="http://purl.obolibrary.org/obo/GAZ_00141556"/>
        <obo:IAO_0000115>An ice-capped island 3.5 mi long that lies 13 mi NNE of Shepard Island, off the Getz Ice Shelf of Marie Byrd Land.</obo:IAO_0000115>
        <oboInOwl:hasOBONamespace>GAZ</oboInOwl:hasOBONamespace>
        <oboInOwl:id>GAZ:00048404</oboInOwl:id>
        <rdfs:label>Forrester Island</rdfs:label>
    </owl:NamedIndividual>
    


    <!-- http://purl.obolibrary.org/obo/GAZ_00048405 -->

    <owl:NamedIndividual rdf:about="http://purl.obolibrary.org/obo/GAZ_00048405">
        <obo:RO_0001025 rdf:resource="http://purl.obolibrary.org/obo/GAZ_00003703"/>
        <obo:IAO_0000115>An ice-covered island about 28 km long and 4-6 km wide, with numerous outcrops exposed along its flanks, extending NNW-SSE, on the eastern side of the Amery Ice Shelf.</obo:IAO_0000115>
        <oboInOwl:hasOBONamespace>GAZ</oboInOwl:hasOBONamespace>
        <oboInOwl:id>GAZ:00048405</oboInOwl:id>
        <rdfs:label>Gillock Island</rdfs:label>
    </owl:NamedIndividual>
    


    <!-- http://purl.obolibrary.org/obo/GAZ_00048406 -->

    <owl:NamedIndividual rdf:about="http://purl.obolibrary.org/obo/GAZ_00048406">
        <obo:RO_0001025 rdf:resource="http://purl.obolibrary.org/obo/GAZ_00004045"/>
        <obo:IAO_0000115>An ice-covered, dome-shaped island lying 6 km east of Cape Rymill, in the Weddell Sea, off the eastern coast of Palmer Land.</obo:IAO_0000115>
        <oboInOwl:hasOBONamespace>GAZ</oboInOwl:hasOBONamespace>
        <oboInOwl:id>GAZ:00048406</oboInOwl:id>
        <rdfs:label>Hearst Island</rdfs:label>
    </owl:NamedIndividual>
    


    <!-- http://purl.obolibrary.org/obo/GAZ_00048407 -->

    <owl:NamedIndividual rdf:about="http://purl.obolibrary.org/obo/GAZ_00048407">
        <obo:RO_0001025 rdf:resource="http://purl.obolibrary.org/obo/GAZ_00051128"/>
        <obo:IAO_0000115>A mountainous island, 21 km long, 10 km wide and rising to 1,000 m, situated in the north-central portion of Hanusse Bay, off the west coast of Graham Land, Antarctica.</obo:IAO_0000115>
        <oboInOwl:hasOBONamespace>GAZ</oboInOwl:hasOBONamespace>
        <oboInOwl:id>GAZ:00048407</oboInOwl:id>
        <rdfs:label>Liard Island</rdfs:label>
    </owl:NamedIndividual>
    


    <!-- http://purl.obolibrary.org/obo/GAZ_00048408 -->

    <owl:NamedIndividual rdf:about="http://purl.obolibrary.org/obo/GAZ_00048408">
        <obo:RO_0001025 rdf:resource="http://purl.obolibrary.org/obo/GAZ_00051129"/>
        <obo:IAO_0000115>An ice-covered island in the West Ice Shelf of Antarctica, rising to 240 m, 11 km southeast of Leskov Island.</obo:IAO_0000115>
        <oboInOwl:hasOBONamespace>GAZ</oboInOwl:hasOBONamespace>
        <oboInOwl:id>GAZ:00048408</oboInOwl:id>
        <rdfs:label>Mikhaylov Island</rdfs:label>
    </owl:NamedIndividual>
    


    <!-- http://purl.obolibrary.org/obo/GAZ_00048409 -->

    <owl:NamedIndividual rdf:about="http://purl.obolibrary.org/obo/GAZ_00048409">
        <obo:RO_0001025 rdf:resource="http://purl.obolibrary.org/obo/GAZ_00141552"/>
        <obo:IAO_0000115>A mountainous island, 27 km long and from 5 to 18 km wide, lying between Bigourdan Fjord and Bourgeois Fjord off the west coast of Graham Land.</obo:IAO_0000115>
        <oboInOwl:hasOBONamespace>GAZ</oboInOwl:hasOBONamespace>
        <oboInOwl:id>GAZ:00048409</oboInOwl:id>
        <rdfs:label>Pourquoi Pas Island</rdfs:label>
    </owl:NamedIndividual>
    


    <!-- http://purl.obolibrary.org/obo/GAZ_00048410 -->

    <owl:NamedIndividual rdf:about="http://purl.obolibrary.org/obo/GAZ_00048410">
        <obo:RO_0001025 rdf:resource="http://purl.obolibrary.org/obo/GAZ_00009523"/>
        <obo:IAO_0000115>A small island in the South Orkney Islands, joined to the S end of Powell Island by a narrow isthmus of occasionally submerged boulders.</obo:IAO_0000115>
        <oboInOwl:hasOBONamespace>GAZ</oboInOwl:hasOBONamespace>
        <oboInOwl:id>GAZ:00048410</oboInOwl:id>
        <rdfs:label>Michelsen Island</rdfs:label>
    </owl:NamedIndividual>
    


    <!-- http://purl.obolibrary.org/obo/GAZ_00048411 -->

    <owl:NamedIndividual rdf:about="http://purl.obolibrary.org/obo/GAZ_00048411">
        <obo:RO_0001025 rdf:resource="http://purl.obolibrary.org/obo/GAZ_00009523"/>
        <obo:IAO_0000115>An island 2.5 mi long and 0.5 mi wide, lying 0.5 mi SE of Powell Island in the South Orkney Islands.</obo:IAO_0000115>
        <oboInOwl:hasOBONamespace>GAZ</oboInOwl:hasOBONamespace>
        <oboInOwl:id>GAZ:00048411</oboInOwl:id>
        <rdfs:label>Fredriksen Island</rdfs:label>
    </owl:NamedIndividual>
    


    <!-- http://purl.obolibrary.org/obo/GAZ_00048412 -->

    <owl:NamedIndividual rdf:about="http://purl.obolibrary.org/obo/GAZ_00048412">
        <obo:RO_0001025 rdf:resource="http://purl.obolibrary.org/obo/GAZ_00009523"/>
        <obo:IAO_0000115>An island 0.6 mi S of Michelsen Island and 1 mi W of the S part of Fredriksen Island, in the South Orkney Islands.</obo:IAO_0000115>
        <oboInOwl:hasOBONamespace>GAZ</oboInOwl:hasOBONamespace>
        <oboInOwl:id>GAZ:00048412</oboInOwl:id>
        <rdfs:label>Grey Island</rdfs:label>
    </owl:NamedIndividual>
    


    <!-- http://purl.obolibrary.org/obo/GAZ_00048413 -->

    <owl:NamedIndividual rdf:about="http://purl.obolibrary.org/obo/GAZ_00048413">
        <obo:RO_0001025 rdf:resource="http://purl.obolibrary.org/obo/GAZ_00051510"/>
        <obo:IAO_0000115>An island 24 miles long, mainly ice covered but surmounted by prominent peaks of Desko Mountains, 5 miles west of the north part of Alexander Island in the north entrance to Wilkins Sound.</obo:IAO_0000115>
        <oboInOwl:hasOBONamespace>GAZ</oboInOwl:hasOBONamespace>
        <oboInOwl:id>GAZ:00048413</oboInOwl:id>
        <rdfs:label>Rothschild Island</rdfs:label>
    </owl:NamedIndividual>
    


    <!-- http://purl.obolibrary.org/obo/GAZ_00048414 -->

    <owl:NamedIndividual rdf:about="http://purl.obolibrary.org/obo/GAZ_00048414">
        <obo:RO_0001025 rdf:resource="http://purl.obolibrary.org/obo/GAZ_00004045"/>
        <obo:IAO_0000115>An almost completely snowcapped island, 32 km long and 10 km wide, lying off the east coast of the Antarctic Peninsula. It is separated from James Ross Island to the northeast by Admiralty Sound.</obo:IAO_0000115>
        <oboInOwl:hasOBONamespace>GAZ</oboInOwl:hasOBONamespace>
        <oboInOwl:id>GAZ:00048414</oboInOwl:id>
        <rdfs:label>Snow Hill Island</rdfs:label>
    </owl:NamedIndividual>
    


    <!-- http://purl.obolibrary.org/obo/GAZ_00048415 -->

    <owl:NamedIndividual rdf:about="http://purl.obolibrary.org/obo/GAZ_00048415">
        <obo:RO_0001025 rdf:resource="http://purl.obolibrary.org/obo/GAZ_00051133"/>
        <obo:IAO_0000115>A snow-covered island, 12 miles long from east to west and 10 miles wide, rising above the Larsen Ice Shelf off the east coast of Palmer Land, 12 miles southeast of Cape Sharbonneau.</obo:IAO_0000115>
        <oboInOwl:hasOBONamespace>GAZ</oboInOwl:hasOBONamespace>
        <oboInOwl:id>GAZ:00048415</oboInOwl:id>
        <rdfs:label>Steele Island</rdfs:label>
    </owl:NamedIndividual>
    


    <!-- http://purl.obolibrary.org/obo/GAZ_00049370 -->

    <owl:NamedIndividual rdf:about="http://purl.obolibrary.org/obo/GAZ_00049370">
        <obo:RO_0001025 rdf:resource="http://purl.obolibrary.org/obo/GAZ_00014094"/>
        <obo:IAO_0000115>A small, isolated reef, which uncovers at low water, lying 0.15 mi SE of Kilhy Island, in the Windmill Islands.</obo:IAO_0000115>
        <oboInOwl:hasOBONamespace>GAZ</oboInOwl:hasOBONamespace>
        <oboInOwl:id>GAZ:00049370</oboInOwl:id>
        <rdfs:label>Kilby Reef</rdfs:label>
    </owl:NamedIndividual>
    


    <!-- http://purl.obolibrary.org/obo/GAZ_00050797 -->

    <owl:NamedIndividual rdf:about="http://purl.obolibrary.org/obo/GAZ_00050797">
        <obo:RO_0001025 rdf:resource="http://purl.obolibrary.org/obo/GAZ_00045057"/>
        <obo:IAO_0000115>A group of islands standing 2.5 km off Mabus Point, Queen Mary Coast.</obo:IAO_0000115>
        <oboInOwl:hasOBONamespace>GAZ</oboInOwl:hasOBONamespace>
        <oboInOwl:id>GAZ:00050797</oboInOwl:id>
        <rdfs:label>Haswell Islands</rdfs:label>
    </owl:NamedIndividual>
    


    <!-- http://purl.obolibrary.org/obo/GAZ_00050798 -->

    <owl:NamedIndividual rdf:about="http://purl.obolibrary.org/obo/GAZ_00050798">
        <obo:RO_0001025 rdf:resource="http://purl.obolibrary.org/obo/GAZ_00050797"/>
        <oboInOwl:hasOBONamespace>GAZ</oboInOwl:hasOBONamespace>
        <oboInOwl:id>GAZ:00050798</oboInOwl:id>
        <rdfs:label>Haswell Island</rdfs:label>
    </owl:NamedIndividual>
    


    <!-- http://purl.obolibrary.org/obo/GAZ_00051124 -->

    <owl:NamedIndividual rdf:about="http://purl.obolibrary.org/obo/GAZ_00051124">
        <obo:RO_0001025 rdf:resource="http://purl.obolibrary.org/obo/GAZ_00023352"/>
        <obo:IAO_0000115>An island.</obo:IAO_0000115>
        <oboInOwl:hasOBONamespace>GAZ</oboInOwl:hasOBONamespace>
        <oboInOwl:id>GAZ:00051124</oboInOwl:id>
        <rdfs:label>Lion Island</rdfs:label>
    </owl:NamedIndividual>
    


    <!-- http://purl.obolibrary.org/obo/GAZ_00051125 -->

    <owl:NamedIndividual rdf:about="http://purl.obolibrary.org/obo/GAZ_00051125">
        <obo:RO_0001025 rdf:resource="http://purl.obolibrary.org/obo/GAZ_00050797"/>
        <oboInOwl:hasOBONamespace>GAZ</oboInOwl:hasOBONamespace>
        <oboInOwl:id>GAZ:00051125</oboInOwl:id>
        <rdfs:label>Zykov Island</rdfs:label>
    </owl:NamedIndividual>
    


    <!-- http://purl.obolibrary.org/obo/GAZ_00051126 -->

    <owl:NamedIndividual rdf:about="http://purl.obolibrary.org/obo/GAZ_00051126">
        <obo:RO_0001025 rdf:resource="http://purl.obolibrary.org/obo/GAZ_00050797"/>
        <oboInOwl:hasOBONamespace>GAZ</oboInOwl:hasOBONamespace>
        <oboInOwl:id>GAZ:00051126</oboInOwl:id>
        <rdfs:label>Fulmar Island</rdfs:label>
    </owl:NamedIndividual>
    


    <!-- http://purl.obolibrary.org/obo/GAZ_00051127 -->

    <owl:NamedIndividual rdf:about="http://purl.obolibrary.org/obo/GAZ_00051127">
        <obo:RO_0001025 rdf:resource="http://purl.obolibrary.org/obo/GAZ_00050797"/>
        <oboInOwl:hasOBONamespace>GAZ</oboInOwl:hasOBONamespace>
        <oboInOwl:id>GAZ:00051127</oboInOwl:id>
        <rdfs:label>Buromskiy Island</rdfs:label>
    </owl:NamedIndividual>
    


    <!-- http://purl.obolibrary.org/obo/GAZ_00051128 -->

    <owl:NamedIndividual rdf:about="http://purl.obolibrary.org/obo/GAZ_00051128">
        <obo:RO_0001025 rdf:resource="http://purl.obolibrary.org/obo/GAZ_00141552"/>
        <obo:IAO_0000115>A broad bay, 32 km long in a general north-south direction, lying between the northern portions of Adelaide Island and Arrowsmith Peninsula.</obo:IAO_0000115>
        <oboInOwl:hasOBONamespace>GAZ</oboInOwl:hasOBONamespace>
        <oboInOwl:id>GAZ:00051128</oboInOwl:id>
        <rdfs:label>Hanusse Bay</rdfs:label>
    </owl:NamedIndividual>
    


    <!-- http://purl.obolibrary.org/obo/GAZ_00051129 -->

    <owl:NamedIndividual rdf:about="http://purl.obolibrary.org/obo/GAZ_00051129">
        <obo:RO_0001025 rdf:resource="http://purl.obolibrary.org/obo/GAZ_00045057"/>
        <obo:IAO_0000115>A prominent ice shelf extending about 288 km in an E-W direction along the Antarctic coast between Barrier Bay and Posadowsky Bay.</obo:IAO_0000115>
        <oboInOwl:hasOBONamespace>GAZ</oboInOwl:hasOBONamespace>
        <oboInOwl:id>GAZ:00051129</oboInOwl:id>
        <rdfs:label>West Ice Shelf</rdfs:label>
    </owl:NamedIndividual>
    


    <!-- http://purl.obolibrary.org/obo/GAZ_00051130 -->

    <owl:NamedIndividual rdf:about="http://purl.obolibrary.org/obo/GAZ_00051130">
        <obo:RO_0001025 rdf:resource="http://purl.obolibrary.org/obo/GAZ_00051129"/>
        <obo:IAO_0000115>An ice-covered island in the West Ice Shelf, rising to 185 m, 6 miles northwest of Mikhaylov Island, off the coast of Antarctica.</obo:IAO_0000115>
        <oboInOwl:hasOBONamespace>GAZ</oboInOwl:hasOBONamespace>
        <oboInOwl:id>GAZ:00051130</oboInOwl:id>
        <rdfs:label>Leskov Island</rdfs:label>
    </owl:NamedIndividual>
    


    <!-- http://purl.obolibrary.org/obo/GAZ_00051132 -->

    <owl:NamedIndividual rdf:about="http://purl.obolibrary.org/obo/GAZ_00051132">
        <obo:RO_0001025 rdf:resource="http://purl.obolibrary.org/obo/GAZ_00045074"/>
        <obo:IAO_0000115>A group of rocky islands and rocks about 95 km long and 9 to 28 km wide, extending in a north-east direction off the Bunger Hills, Knox Coast, Wilkes Lane.</obo:IAO_0000115>
        <oboInOwl:hasOBONamespace>GAZ</oboInOwl:hasOBONamespace>
        <oboInOwl:id>GAZ:00051132</oboInOwl:id>
        <rdfs:label>Highjump Archipelago</rdfs:label>
    </owl:NamedIndividual>
    


    <!-- http://purl.obolibrary.org/obo/GAZ_00051133 -->

    <owl:NamedIndividual rdf:about="http://purl.obolibrary.org/obo/GAZ_00051133">
        <obo:RO_0001025 rdf:resource="http://purl.obolibrary.org/obo/GAZ_00004045"/>
        <obo:IAO_0000115>A long, fringing ice shelf in the northwest part of the Weddell Sea, extending along the east coast of Antarctic Peninsula from Cape Longing to the area just southward of Hearst Island.</obo:IAO_0000115>
        <oboInOwl:hasOBONamespace>GAZ</oboInOwl:hasOBONamespace>
        <oboInOwl:id>GAZ:00051133</oboInOwl:id>
        <rdfs:label>Larsen Ice Shelf</rdfs:label>
    </owl:NamedIndividual>
    


    <!-- http://purl.obolibrary.org/obo/GAZ_00051134 -->

    <owl:NamedIndividual rdf:about="http://purl.obolibrary.org/obo/GAZ_00051134">
        <obo:RO_0001025 rdf:resource="http://purl.obolibrary.org/obo/GAZ_00007425"/>
        <obo:IAO_0000115>A small peninsula separating Marian and Potter Coves at the southwest end of King George Island, in the South Shetland Islands.</obo:IAO_0000115>
        <oboInOwl:hasOBONamespace>GAZ</oboInOwl:hasOBONamespace>
        <oboInOwl:id>GAZ:00051134</oboInOwl:id>
        <rdfs:label>Barton Peninsula</rdfs:label>
    </owl:NamedIndividual>
    


    <!-- http://purl.obolibrary.org/obo/GAZ_00051498 -->

    <owl:NamedIndividual rdf:about="http://purl.obolibrary.org/obo/GAZ_00051498">
        <rdf:type rdf:resource="http://purl.obolibrary.org/obo/ENVO_00000016"/>
        <obo:RO_0001025 rdf:resource="http://purl.obolibrary.org/obo/GAZ_00000373"/>
        <obo:IAO_0000115>A marginal sea extending from 20degE and 45degE, the limits of Dronning Maud Land. No definitive N boundary.</obo:IAO_0000115>
        <oboInOwl:hasOBONamespace>GAZ</oboInOwl:hasOBONamespace>
        <oboInOwl:id>GAZ:00051498</oboInOwl:id>
        <rdfs:label>King Haakon VII Sea</rdfs:label>
    </owl:NamedIndividual>
    


    <!-- http://purl.obolibrary.org/obo/GAZ_00051499 -->

    <owl:NamedIndividual rdf:about="http://purl.obolibrary.org/obo/GAZ_00051499">
        <obo:RO_0001025 rdf:resource="http://purl.obolibrary.org/obo/GAZ_00000373"/>
        <obo:IAO_0000115>A coastal sea of East Antarctica. From the limit of the Mawson Sea at approximately 113degE to Cape Adare at 170degE. No definitive N boundary.</obo:IAO_0000115>
        <oboInOwl:hasOBONamespace>GAZ</oboInOwl:hasOBONamespace>
        <oboInOwl:id>GAZ:00051499</oboInOwl:id>
        <rdfs:label>Dumont d&apos;Urville Sea</rdfs:label>
    </owl:NamedIndividual>
    


    <!-- http://purl.obolibrary.org/obo/GAZ_00051500 -->

    <owl:NamedIndividual rdf:about="http://purl.obolibrary.org/obo/GAZ_00051500">
        <obo:RO_0001025 rdf:resource="http://purl.obolibrary.org/obo/GAZ_00051498"/>
        <obo:IAO_0000115>A coastal sea off East Antarctica, between Riiser-Larsen Halvoya at 34degE and Tange Promontory at 46.5degE, bordered by Prins Harald Kyst and Kronprins Olv Kyst. No definitive N boundary.</obo:IAO_0000115>
        <oboInOwl:hasOBONamespace>GAZ</oboInOwl:hasOBONamespace>
        <oboInOwl:id>GAZ:00051500</oboInOwl:id>
        <rdfs:label>Cosmonaut Sea</rdfs:label>
    </owl:NamedIndividual>
    


    <!-- http://purl.obolibrary.org/obo/GAZ_00051503 -->

    <owl:NamedIndividual rdf:about="http://purl.obolibrary.org/obo/GAZ_00051503">
        <obo:RO_0001025 rdf:resource="http://purl.obolibrary.org/obo/GAZ_00014085"/>
        <obo:IAO_0000115>An ice-filled sound, 216 km long and 64 km wide, separating Thurston Island from the Eights Coast of Ellsworth Land in Antarctica. The sound is occupied by the western part of the Abbot Ice Shelf.</obo:IAO_0000115>
        <oboInOwl:hasOBONamespace>GAZ</oboInOwl:hasOBONamespace>
        <oboInOwl:id>GAZ:00051503</oboInOwl:id>
        <rdfs:label>Peacock Sound</rdfs:label>
    </owl:NamedIndividual>
    


    <!-- http://purl.obolibrary.org/obo/GAZ_00051504 -->

    <owl:NamedIndividual rdf:about="http://purl.obolibrary.org/obo/GAZ_00051504">
        <obo:RO_0001025 rdf:resource="http://purl.obolibrary.org/obo/GAZ_00014085"/>
        <obo:RO_0001025 rdf:resource="http://purl.obolibrary.org/obo/GAZ_00051503"/>
        <obo:IAO_0000115>An ice shelf 400 km long and 64 km wide, bordering Eights Coast from Cape Waite to Phrogner Point in Antarctica. Thurston Island lies along the northern edge of the western half of this ice shelf; other sizable islands (Sherman, Carpenter, Dustin, Johnson, McNamara, Farwell and Dendtler) lie partly or wholly within it.</obo:IAO_0000115>
        <oboInOwl:hasOBONamespace>GAZ</oboInOwl:hasOBONamespace>
        <oboInOwl:id>GAZ:00051504</oboInOwl:id>
        <rdfs:label>Abbot Ice Shelf</rdfs:label>
    </owl:NamedIndividual>
    


    <!-- http://purl.obolibrary.org/obo/GAZ_00051505 -->

    <owl:NamedIndividual rdf:about="http://purl.obolibrary.org/obo/GAZ_00051505">
        <obo:RO_0001025 rdf:resource="http://purl.obolibrary.org/obo/GAZ_00051504"/>
        <oboInOwl:hasOBONamespace>GAZ</oboInOwl:hasOBONamespace>
        <oboInOwl:id>GAZ:00051505</oboInOwl:id>
        <rdfs:label>Carpenter Island</rdfs:label>
    </owl:NamedIndividual>
    


    <!-- http://purl.obolibrary.org/obo/GAZ_00051506 -->

    <owl:NamedIndividual rdf:about="http://purl.obolibrary.org/obo/GAZ_00051506">
        <obo:RO_0001025 rdf:resource="http://purl.obolibrary.org/obo/GAZ_00051504"/>
        <oboInOwl:hasOBONamespace>GAZ</oboInOwl:hasOBONamespace>
        <oboInOwl:id>GAZ:00051506</oboInOwl:id>
        <rdfs:label>Johnson Island</rdfs:label>
    </owl:NamedIndividual>
    


    <!-- http://purl.obolibrary.org/obo/GAZ_00051507 -->

    <owl:NamedIndividual rdf:about="http://purl.obolibrary.org/obo/GAZ_00051507">
        <obo:RO_0001025 rdf:resource="http://purl.obolibrary.org/obo/GAZ_00051504"/>
        <oboInOwl:hasOBONamespace>GAZ</oboInOwl:hasOBONamespace>
        <oboInOwl:id>GAZ:00051507</oboInOwl:id>
        <rdfs:label>Farwell Island</rdfs:label>
    </owl:NamedIndividual>
    


    <!-- http://purl.obolibrary.org/obo/GAZ_00051508 -->

    <owl:NamedIndividual rdf:about="http://purl.obolibrary.org/obo/GAZ_00051508">
        <obo:RO_0001025 rdf:resource="http://purl.obolibrary.org/obo/GAZ_00051504"/>
        <oboInOwl:hasOBONamespace>GAZ</oboInOwl:hasOBONamespace>
        <oboInOwl:id>GAZ:00051508</oboInOwl:id>
        <rdfs:label>Dendtler Island</rdfs:label>
    </owl:NamedIndividual>
    


    <!-- http://purl.obolibrary.org/obo/GAZ_00051509 -->

    <owl:NamedIndividual rdf:about="http://purl.obolibrary.org/obo/GAZ_00051509">
        <obo:RO_0001025 rdf:resource="http://purl.obolibrary.org/obo/GAZ_00051504"/>
        <oboInOwl:hasOBONamespace>GAZ</oboInOwl:hasOBONamespace>
        <oboInOwl:id>GAZ:00051509</oboInOwl:id>
        <rdfs:label>McNamara Island</rdfs:label>
    </owl:NamedIndividual>
    


    <!-- http://purl.obolibrary.org/obo/GAZ_00051510 -->

    <owl:NamedIndividual rdf:about="http://purl.obolibrary.org/obo/GAZ_00051510">
        <obo:RO_0001025 rdf:resource="http://purl.obolibrary.org/obo/GAZ_00014084"/>
        <obo:IAO_0000115>A sound that is largely occupied by the Wilkins Ice Shelf; it is located between the concave western coastline of Alexander Island and the shores of Charcot Island and Latady Island farther to the west.</obo:IAO_0000115>
        <oboInOwl:hasOBONamespace>GAZ</oboInOwl:hasOBONamespace>
        <oboInOwl:id>GAZ:00051510</oboInOwl:id>
        <rdfs:label>Wilkins Sound</rdfs:label>
    </owl:NamedIndividual>
    


    <!-- http://purl.obolibrary.org/obo/GAZ_00051511 -->

    <owl:NamedIndividual rdf:about="http://purl.obolibrary.org/obo/GAZ_00051511">
        <obo:RO_0001025 rdf:resource="http://purl.obolibrary.org/obo/GAZ_00051510"/>
        <obo:IAO_0000115>A rectangular ice shelf about 80 miles long and 60 miles wide. The feature occupies the central part of Wilkins Sound.</obo:IAO_0000115>
        <oboInOwl:hasOBONamespace>GAZ</oboInOwl:hasOBONamespace>
        <oboInOwl:id>GAZ:00051511</oboInOwl:id>
        <rdfs:label>Wilkins Ice Shelf</rdfs:label>
    </owl:NamedIndividual>
    


    <!-- http://purl.obolibrary.org/obo/GAZ_00051512 -->

    <owl:NamedIndividual rdf:about="http://purl.obolibrary.org/obo/GAZ_00051512">
        <obo:RO_0001025 rdf:resource="http://purl.obolibrary.org/obo/GAZ_00014122"/>
        <oboInOwl:hasOBONamespace>GAZ</oboInOwl:hasOBONamespace>
        <oboInOwl:id>GAZ:00051512</oboInOwl:id>
        <rdfs:label>Dannebrog Islands</rdfs:label>
    </owl:NamedIndividual>
    


    <!-- http://purl.obolibrary.org/obo/GAZ_00051513 -->

    <owl:NamedIndividual rdf:about="http://purl.obolibrary.org/obo/GAZ_00051513">
        <obo:RO_0001025 rdf:resource="http://purl.obolibrary.org/obo/GAZ_00014122"/>
        <oboInOwl:hasOBONamespace>GAZ</oboInOwl:hasOBONamespace>
        <oboInOwl:id>GAZ:00051513</oboInOwl:id>
        <rdfs:label>Plenau island</rdfs:label>
    </owl:NamedIndividual>
    


    <!-- http://purl.obolibrary.org/obo/GAZ_00051514 -->

    <owl:NamedIndividual rdf:about="http://purl.obolibrary.org/obo/GAZ_00051514">
        <obo:RO_0001025 rdf:resource="http://purl.obolibrary.org/obo/GAZ_00014122"/>
        <oboInOwl:hasOBONamespace>GAZ</oboInOwl:hasOBONamespace>
        <oboInOwl:id>GAZ:00051514</oboInOwl:id>
        <rdfs:label>Wauwerman Islands</rdfs:label>
    </owl:NamedIndividual>
    


    <!-- http://purl.obolibrary.org/obo/GAZ_00051515 -->

    <owl:NamedIndividual rdf:about="http://purl.obolibrary.org/obo/GAZ_00051515">
        <obo:RO_0001025 rdf:resource="http://purl.obolibrary.org/obo/GAZ_00014122"/>
        <oboInOwl:hasOBONamespace>GAZ</oboInOwl:hasOBONamespace>
        <oboInOwl:id>GAZ:00051515</oboInOwl:id>
        <rdfs:label>Myriad Islands</rdfs:label>
    </owl:NamedIndividual>
    


    <!-- http://purl.obolibrary.org/obo/GAZ_00051516 -->

    <owl:NamedIndividual rdf:about="http://purl.obolibrary.org/obo/GAZ_00051516">
        <obo:RO_0001025 rdf:resource="http://purl.obolibrary.org/obo/GAZ_00014122"/>
        <oboInOwl:hasOBONamespace>GAZ</oboInOwl:hasOBONamespace>
        <oboInOwl:id>GAZ:00051516</oboInOwl:id>
        <rdfs:label>Jalaur Islands</rdfs:label>
    </owl:NamedIndividual>
    


    <!-- http://purl.obolibrary.org/obo/GAZ_00051517 -->

    <owl:NamedIndividual rdf:about="http://purl.obolibrary.org/obo/GAZ_00051517">
        <obo:RO_0001025 rdf:resource="http://purl.obolibrary.org/obo/GAZ_00014122"/>
        <oboInOwl:hasOBONamespace>GAZ</oboInOwl:hasOBONamespace>
        <oboInOwl:id>GAZ:00051517</oboInOwl:id>
        <rdfs:label>Petermann Islands</rdfs:label>
    </owl:NamedIndividual>
    


    <!-- http://purl.obolibrary.org/obo/GAZ_00051518 -->

    <owl:NamedIndividual rdf:about="http://purl.obolibrary.org/obo/GAZ_00051518">
        <obo:RO_0001025 rdf:resource="http://purl.obolibrary.org/obo/GAZ_00014122"/>
        <obo:IAO_0000115>A group of islands.</obo:IAO_0000115>
        <oboInOwl:hasOBONamespace>GAZ</oboInOwl:hasOBONamespace>
        <oboInOwl:id>GAZ:00051518</oboInOwl:id>
        <rdfs:label>Argentine Islands</rdfs:label>
    </owl:NamedIndividual>
    


    <!-- http://purl.obolibrary.org/obo/GAZ_00051519 -->

    <owl:NamedIndividual rdf:about="http://purl.obolibrary.org/obo/GAZ_00051519">
        <obo:RO_0001025 rdf:resource="http://purl.obolibrary.org/obo/GAZ_00014122"/>
        <oboInOwl:hasOBONamespace>GAZ</oboInOwl:hasOBONamespace>
        <oboInOwl:id>GAZ:00051519</oboInOwl:id>
        <rdfs:label>Betbeder Islands</rdfs:label>
    </owl:NamedIndividual>
    


    <!-- http://purl.obolibrary.org/obo/GAZ_00051520 -->

    <owl:NamedIndividual rdf:about="http://purl.obolibrary.org/obo/GAZ_00051520">
        <obo:RO_0001025 rdf:resource="http://purl.obolibrary.org/obo/GAZ_00014089"/>
        <obo:IAO_0000115>A small group of islands and rocks lying off the southeast coast of Adelaide Island, 3 km SE of the Leonie Islands.</obo:IAO_0000115>
        <oboInOwl:hasOBONamespace>GAZ</oboInOwl:hasOBONamespace>
        <oboInOwl:id>GAZ:00051520</oboInOwl:id>
        <rdfs:label>Mikkelsen Islands</rdfs:label>
    </owl:NamedIndividual>
    


    <!-- http://purl.obolibrary.org/obo/GAZ_00051521 -->

    <owl:NamedIndividual rdf:about="http://purl.obolibrary.org/obo/GAZ_00051521">
        <obo:RO_0001025 rdf:resource="http://purl.obolibrary.org/obo/GAZ_00141023"/>
        <obo:IAO_0000115>An ice island in the Mawson Sea 160 km off the East Antarctica Coast of Queen Mary Land, Australian Antarctic Territory, that exists periodically.</obo:IAO_0000115>
        <oboInOwl:hasOBONamespace>GAZ</oboInOwl:hasOBONamespace>
        <oboInOwl:id>GAZ:00051521</oboInOwl:id>
        <rdfs:label>Pobeda Ice Island</rdfs:label>
    </owl:NamedIndividual>
    


    <!-- http://purl.obolibrary.org/obo/GAZ_00051522 -->

    <owl:NamedIndividual rdf:about="http://purl.obolibrary.org/obo/GAZ_00051522">
        <obo:RO_0001025 rdf:resource="http://purl.obolibrary.org/obo/GAZ_00023352"/>
        <obo:IAO_0000115>An island.</obo:IAO_0000115>
        <oboInOwl:hasOBONamespace>GAZ</oboInOwl:hasOBONamespace>
        <oboInOwl:id>GAZ:00051522</oboInOwl:id>
        <rdfs:label>Ile des Petrels</rdfs:label>
    </owl:NamedIndividual>
    


    <!-- http://purl.obolibrary.org/obo/GAZ_00051523 -->

    <owl:NamedIndividual rdf:about="http://purl.obolibrary.org/obo/GAZ_00051523">
        <obo:RO_0001025 rdf:resource="http://purl.obolibrary.org/obo/GAZ_00139422"/>
        <obo:IAO_0000115>Numerous small rocky islands centered 1 mi NW of Byrd Head, just E of Taylor Glacier.</obo:IAO_0000115>
        <oboInOwl:hasOBONamespace>GAZ</oboInOwl:hasOBONamespace>
        <oboInOwl:id>GAZ:00051523</oboInOwl:id>
        <rdfs:label>Colbeck Archipelago</rdfs:label>
    </owl:NamedIndividual>
    


    <!-- http://purl.obolibrary.org/obo/GAZ_00051524 -->

    <owl:NamedIndividual rdf:about="http://purl.obolibrary.org/obo/GAZ_00051524">
        <obo:RO_0001025 rdf:resource="http://purl.obolibrary.org/obo/GAZ_00051499"/>
        <obo:IAO_0000115>Small group of rocky islands lying close off Cape Decouverte, Adelie Coast.</obo:IAO_0000115>
        <oboInOwl:hasOBONamespace>GAZ</oboInOwl:hasOBONamespace>
        <oboInOwl:id>GAZ:00051524</oboInOwl:id>
        <rdfs:label>Curzon Islands</rdfs:label>
    </owl:NamedIndividual>
    


    <!-- http://purl.obolibrary.org/obo/GAZ_00051525 -->

    <owl:NamedIndividual rdf:about="http://purl.obolibrary.org/obo/GAZ_00051525">
        <obo:RO_0001025 rdf:resource="http://purl.obolibrary.org/obo/GAZ_00023304"/>
        <obo:IAO_0000115>A group of small volcanic islands lying off the coast of Victoria Land, 5 mi NE of Cape Chocolate, in the N part of the ice shelf bordering McMurdo Sound.</obo:IAO_0000115>
        <oboInOwl:hasOBONamespace>GAZ</oboInOwl:hasOBONamespace>
        <oboInOwl:id>GAZ:00051525</oboInOwl:id>
        <rdfs:label>Dailey Islands</rdfs:label>
    </owl:NamedIndividual>
    


    <!-- http://purl.obolibrary.org/obo/GAZ_00051526 -->

    <owl:NamedIndividual rdf:about="http://purl.obolibrary.org/obo/GAZ_00051526">
        <obo:RO_0001025 rdf:resource="http://purl.obolibrary.org/obo/GAZ_00023304"/>
        <obo:IAO_0000115>An extensive group of large ice-covered islands within Sulzberger Ice Shelf.</obo:IAO_0000115>
        <oboInOwl:hasOBONamespace>GAZ</oboInOwl:hasOBONamespace>
        <oboInOwl:id>GAZ:00051526</oboInOwl:id>
        <rdfs:label>Marshall Archipelago</rdfs:label>
    </owl:NamedIndividual>
    


    <!-- http://purl.obolibrary.org/obo/GAZ_00051527 -->

    <owl:NamedIndividual rdf:about="http://purl.obolibrary.org/obo/GAZ_00051527">
        <obo:RO_0001025 rdf:resource="http://purl.obolibrary.org/obo/GAZ_00004380"/>
        <obo:RO_0001025 rdf:resource="http://purl.obolibrary.org/obo/GAZ_00051528"/>
        <obo:IAO_0000115>A group of many low, ice-covered islands lying near the center of Dallmann Bay in the Palmer Archipelago.</obo:IAO_0000115>
        <oboInOwl:hasOBONamespace>GAZ</oboInOwl:hasOBONamespace>
        <oboInOwl:id>GAZ:00051527</oboInOwl:id>
        <rdfs:label>Melchior Islands</rdfs:label>
    </owl:NamedIndividual>
    


    <!-- http://purl.obolibrary.org/obo/GAZ_00051528 -->

    <owl:NamedIndividual rdf:about="http://purl.obolibrary.org/obo/GAZ_00051528">
        <obo:RO_0001025 rdf:resource="http://purl.obolibrary.org/obo/GAZ_00141552"/>
        <obo:IAO_0000115>A bay between Anvers Island and Brabant Island.</obo:IAO_0000115>
        <oboInOwl:hasOBONamespace>GAZ</oboInOwl:hasOBONamespace>
        <oboInOwl:id>GAZ:00051528</oboInOwl:id>
        <rdfs:label>Dallmann Bay</rdfs:label>
    </owl:NamedIndividual>
    


    <!-- http://purl.obolibrary.org/obo/GAZ_00051529 -->

    <owl:NamedIndividual rdf:about="http://purl.obolibrary.org/obo/GAZ_00051529">
        <obo:RO_0001025 rdf:resource="http://purl.obolibrary.org/obo/GAZ_00051499"/>
        <obo:IAO_0000115>More than 120 small islands and rocks, of which the largest is Stillwell Island, distributed close off shore in the form of an arc. The archipelago extends from the vicinity of Cape Gray, at the east side of the entrance to Commonwealth Bay, to the vicinity of Garnet Point, at the west side of the entrance to Watt Bay.</obo:IAO_0000115>
        <oboInOwl:hasOBONamespace>GAZ</oboInOwl:hasOBONamespace>
        <oboInOwl:id>GAZ:00051529</oboInOwl:id>
        <rdfs:label>Way Archipelago</rdfs:label>
    </owl:NamedIndividual>
    


    <!-- http://purl.obolibrary.org/obo/GAZ_00051530 -->

    <owl:NamedIndividual rdf:about="http://purl.obolibrary.org/obo/GAZ_00051530">
        <obo:RO_0001025 rdf:resource="http://purl.obolibrary.org/obo/GAZ_00051529"/>
        <oboInOwl:hasOBONamespace>GAZ</oboInOwl:hasOBONamespace>
        <oboInOwl:id>GAZ:00051530</oboInOwl:id>
        <rdfs:label>Stillwell Island</rdfs:label>
    </owl:NamedIndividual>
    


    <!-- http://purl.obolibrary.org/obo/GAZ_00051531 -->

    <owl:NamedIndividual rdf:about="http://purl.obolibrary.org/obo/GAZ_00051531">
        <obo:RO_0001025 rdf:resource="http://purl.obolibrary.org/obo/GAZ_00004380"/>
        <obo:IAO_0000115>A group of small ice-covered islands and rocks which lie W of The Sound in the Melchior Islands, Palmer Archipelago. The islands E of The Sound are called East Melchior Islands.</obo:IAO_0000115>
        <oboInOwl:hasOBONamespace>GAZ</oboInOwl:hasOBONamespace>
        <oboInOwl:id>GAZ:00051531</oboInOwl:id>
        <rdfs:label>West Melchior Islands</rdfs:label>
    </owl:NamedIndividual>
    


    <!-- http://purl.obolibrary.org/obo/GAZ_00051532 -->

    <owl:NamedIndividual rdf:about="http://purl.obolibrary.org/obo/GAZ_00051532">
        <obo:RO_0001025 rdf:resource="http://purl.obolibrary.org/obo/GAZ_00139422"/>
        <obo:IAO_0000115>A group of islands which extends northward from the coast just E of William Scoresby Bay.</obo:IAO_0000115>
        <oboInOwl:hasOBONamespace>GAZ</oboInOwl:hasOBONamespace>
        <oboInOwl:id>GAZ:00051532</oboInOwl:id>
        <rdfs:label>William Scoresby Archipelago</rdfs:label>
    </owl:NamedIndividual>
    


    <!-- http://purl.obolibrary.org/obo/GAZ_00051533 -->

    <owl:NamedIndividual rdf:about="http://purl.obolibrary.org/obo/GAZ_00051533">
        <obo:RO_0001025 rdf:resource="http://purl.obolibrary.org/obo/GAZ_00051532"/>
        <oboInOwl:hasOBONamespace>GAZ</oboInOwl:hasOBONamespace>
        <oboInOwl:id>GAZ:00051533</oboInOwl:id>
        <rdfs:label>Islay Island</rdfs:label>
    </owl:NamedIndividual>
    


    <!-- http://purl.obolibrary.org/obo/GAZ_00051534 -->

    <owl:NamedIndividual rdf:about="http://purl.obolibrary.org/obo/GAZ_00051534">
        <obo:RO_0001025 rdf:resource="http://purl.obolibrary.org/obo/GAZ_00051532"/>
        <oboInOwl:hasOBONamespace>GAZ</oboInOwl:hasOBONamespace>
        <oboInOwl:id>GAZ:00051534</oboInOwl:id>
        <rdfs:label>Couling Island</rdfs:label>
    </owl:NamedIndividual>
    


    <!-- http://purl.obolibrary.org/obo/GAZ_00051535 -->

    <owl:NamedIndividual rdf:about="http://purl.obolibrary.org/obo/GAZ_00051535">
        <obo:RO_0001025 rdf:resource="http://purl.obolibrary.org/obo/GAZ_00051532"/>
        <oboInOwl:hasOBONamespace>GAZ</oboInOwl:hasOBONamespace>
        <oboInOwl:id>GAZ:00051535</oboInOwl:id>
        <rdfs:label>Sheehan Island</rdfs:label>
    </owl:NamedIndividual>
    


    <!-- http://purl.obolibrary.org/obo/GAZ_00051536 -->

    <owl:NamedIndividual rdf:about="http://purl.obolibrary.org/obo/GAZ_00051536">
        <obo:RO_0001025 rdf:resource="http://purl.obolibrary.org/obo/GAZ_00051532"/>
        <oboInOwl:hasOBONamespace>GAZ</oboInOwl:hasOBONamespace>
        <oboInOwl:id>GAZ:00051536</oboInOwl:id>
        <rdfs:label>Bertha Island</rdfs:label>
    </owl:NamedIndividual>
    


    <!-- http://purl.obolibrary.org/obo/GAZ_00051551 -->

    <owl:NamedIndividual rdf:about="http://purl.obolibrary.org/obo/GAZ_00051551">
        <obo:RO_0001025 rdf:resource="http://purl.obolibrary.org/obo/GAZ_00051499"/>
        <obo:IAO_0000115>A group of islands lying just outside the entrance to Yule Bay, Victoria Land.</obo:IAO_0000115>
        <oboInOwl:hasOBONamespace>GAZ</oboInOwl:hasOBONamespace>
        <oboInOwl:id>GAZ:00051551</oboInOwl:id>
        <rdfs:label>Lyall Islands</rdfs:label>
    </owl:NamedIndividual>
    


    <!-- http://purl.obolibrary.org/obo/GAZ_00051552 -->

    <owl:NamedIndividual rdf:about="http://purl.obolibrary.org/obo/GAZ_00051552">
        <obo:RO_0001025 rdf:resource="http://purl.obolibrary.org/obo/GAZ_00051551"/>
        <obo:IAO_0000115>A small, ice-covered island, one of the Lyall Islands, lying 4 miles NNE of Cape Dayman, off the N coast of Victoria Land.</obo:IAO_0000115>
        <oboInOwl:hasOBONamespace>GAZ</oboInOwl:hasOBONamespace>
        <oboInOwl:id>GAZ:00051552</oboInOwl:id>
        <rdfs:label>Novosad Island</rdfs:label>
    </owl:NamedIndividual>
    


    <!-- http://purl.obolibrary.org/obo/GAZ_00051553 -->

    <owl:NamedIndividual rdf:about="http://purl.obolibrary.org/obo/GAZ_00051553">
        <obo:RO_0001025 rdf:resource="http://purl.obolibrary.org/obo/GAZ_00051551"/>
        <obo:IAO_0000115>The largest of the Lyall Islands, lying 4 miles ESE of Cape Hooker off the N coast of Victoria Land.</obo:IAO_0000115>
        <oboInOwl:hasOBONamespace>GAZ</oboInOwl:hasOBONamespace>
        <oboInOwl:id>GAZ:00051553</oboInOwl:id>
        <rdfs:label>Surgeon Island</rdfs:label>
    </owl:NamedIndividual>
    


    <!-- http://purl.obolibrary.org/obo/GAZ_00051554 -->

    <owl:NamedIndividual rdf:about="http://purl.obolibrary.org/obo/GAZ_00051554">
        <obo:RO_0001025 rdf:resource="http://purl.obolibrary.org/obo/GAZ_00051551"/>
        <obo:IAO_0000115>A small ice-covered island, the easternmost of the Lyall Islands, lying just outside the E part of the entrance to Yule Bay, Victoria Land.</obo:IAO_0000115>
        <oboInOwl:hasOBONamespace>GAZ</oboInOwl:hasOBONamespace>
        <oboInOwl:id>GAZ:00051554</oboInOwl:id>
        <rdfs:label>Hughes Island</rdfs:label>
    </owl:NamedIndividual>
    


    <!-- http://purl.obolibrary.org/obo/GAZ_00051555 -->

    <owl:NamedIndividual rdf:about="http://purl.obolibrary.org/obo/GAZ_00051555">
        <obo:RO_0001025 rdf:resource="http://purl.obolibrary.org/obo/GAZ_00051551"/>
        <obo:IAO_0000115>A small, ice-free island of Antarctica. Lying 4 miles to the southeast of the Cape Hooker, it is the westernmost of the Lyall Islands.</obo:IAO_0000115>
        <oboInOwl:hasOBONamespace>GAZ</oboInOwl:hasOBONamespace>
        <oboInOwl:id>GAZ:00051555</oboInOwl:id>
        <rdfs:label>Unger Island</rdfs:label>
    </owl:NamedIndividual>
    


    <!-- http://purl.obolibrary.org/obo/GAZ_00051745 -->

    <owl:NamedIndividual rdf:about="http://purl.obolibrary.org/obo/GAZ_00051745">
        <obo:RO_0001025 rdf:resource="http://purl.obolibrary.org/obo/GAZ_00139422"/>
        <obo:IAO_0000115>A bay indenting the coast for 10 miles between Law Promontory and Fold Island.</obo:IAO_0000115>
        <oboInOwl:hasOBONamespace>GAZ</oboInOwl:hasOBONamespace>
        <oboInOwl:id>GAZ:00051745</oboInOwl:id>
        <rdfs:label>Stefansson Bay</rdfs:label>
    </owl:NamedIndividual>
    


    <!-- http://purl.obolibrary.org/obo/GAZ_00051746 -->

    <owl:NamedIndividual rdf:about="http://purl.obolibrary.org/obo/GAZ_00051746">
        <obo:RO_0001025 rdf:resource="http://purl.obolibrary.org/obo/GAZ_00051745"/>
        <obo:IAO_0000115>A group of small islands lying off the E end of Law Promontory, at the West side of the entrance to Stefansson Bay.</obo:IAO_0000115>
        <oboInOwl:hasOBONamespace>GAZ</oboInOwl:hasOBONamespace>
        <oboInOwl:id>GAZ:00051746</oboInOwl:id>
        <rdfs:label>Law Islands</rdfs:label>
    </owl:NamedIndividual>
    


    <!-- http://purl.obolibrary.org/obo/GAZ_00051747 -->

    <owl:NamedIndividual rdf:about="http://purl.obolibrary.org/obo/GAZ_00051747">
        <obo:RO_0001025 rdf:resource="http://purl.obolibrary.org/obo/GAZ_00139422"/>
        <obo:IAO_0000115>An offshore island, 6 mi long and 3 mi wide, which with smaller islands close southward separate Stefansson Bay to the W from William Scoresby Bay to the east.</obo:IAO_0000115>
        <oboInOwl:hasOBONamespace>GAZ</oboInOwl:hasOBONamespace>
        <oboInOwl:id>GAZ:00051747</oboInOwl:id>
        <rdfs:label>Fold Island</rdfs:label>
    </owl:NamedIndividual>
    


    <!-- http://purl.obolibrary.org/obo/GAZ_00051770 -->

    <owl:NamedIndividual rdf:about="http://purl.obolibrary.org/obo/GAZ_00051770">
        <obo:RO_0001025 rdf:resource="http://purl.obolibrary.org/obo/GAZ_00141552"/>
        <obo:IAO_0000115>A group of small islands lying immediately off the N extremity of Renaud Island, at the N end of the Biscoe Islands.</obo:IAO_0000115>
        <oboInOwl:hasOBONamespace>GAZ</oboInOwl:hasOBONamespace>
        <oboInOwl:id>GAZ:00051770</oboInOwl:id>
        <rdfs:label>Pitt Islands</rdfs:label>
    </owl:NamedIndividual>
    


    <!-- http://purl.obolibrary.org/obo/GAZ_00051957 -->

    <owl:NamedIndividual rdf:about="http://purl.obolibrary.org/obo/GAZ_00051957">
        <obo:RO_0001025 rdf:resource="http://purl.obolibrary.org/obo/GAZ_00004057"/>
        <obo:IAO_0000115>A large shield volcano that forms the eastern part of Ross Island. It has numerous cinder cones and domes on the flanks of the shield and is mostly under snow and ice.</obo:IAO_0000115>
        <oboInOwl:hasOBONamespace>GAZ</oboInOwl:hasOBONamespace>
        <oboInOwl:id>GAZ:00051957</oboInOwl:id>
        <rdfs:label>Mount Terror</rdfs:label>
    </owl:NamedIndividual>
    


    <!-- http://purl.obolibrary.org/obo/GAZ_00051987 -->

    <owl:NamedIndividual rdf:about="http://purl.obolibrary.org/obo/GAZ_00051987">
        <obo:RO_0001025 rdf:resource="http://purl.obolibrary.org/obo/GAZ_00051133"/>
        <obo:IAO_0000115>A group of 16 nunataks emerging from the Larsen Ice Shelf east of Graham Land Peninsula. The Seal Nunataks have been described as separate volcanic vents or remnants of a large shield volcano. Fumarolic activity was reported from Murdoch and Dallman cones in 1982, and fresh-looking pyroclastics and a lava flow at Dallman (not observed in 1979) were seen on the ice surface three years later (Gonzalez-Ferran 1983). Fumarolic activity was observed at Christensen in 1893, and Lindenberg was observed in eruption in 1893. Baker (1968) saw cinders on the ice surface, suggesting a 20th-century eruption. A 1988 British expedition noted that tephra away from nunataks was found only in ice-cored moraines, suggesting a glacial rather than pyroclastic origin. They noted no fumarolic activity, although water vapor resulting from radiant heating of ice-cored moraines was observed.</obo:IAO_0000115>
        <oboInOwl:hasOBONamespace>GAZ</oboInOwl:hasOBONamespace>
        <oboInOwl:id>GAZ:00051987</oboInOwl:id>
        <rdfs:label>Seal Nunataks Volcano</rdfs:label>
    </owl:NamedIndividual>
    


    <!-- http://purl.obolibrary.org/obo/GAZ_00051993 -->

    <owl:NamedIndividual rdf:about="http://purl.obolibrary.org/obo/GAZ_00051993">
        <obo:RO_0001025 rdf:resource="http://purl.obolibrary.org/obo/GAZ_00017731"/>
        <obo:IAO_0000115>A basaltic scoria cone with a 350-m-wide well-preserved summit crater that forms the 180 m high summit on the SW side of the island. A small plug of basaltic lava occupies the 75-m-deep crater. Petrel Crater, a 300-m-wide maar, is located near the east coast. The formation of Deacon Peak scoria cone was dated by lichenometry at about 300 years ago, and the younger Petrel Crater maar was dated at about 100 years (Birkenmajer 1979). Some of the historical reports of fumarolic activity on nearby Bridgeman Island are attributed to the more youthful Penguin Island.</obo:IAO_0000115>
        <oboInOwl:hasOBONamespace>GAZ</oboInOwl:hasOBONamespace>
        <oboInOwl:id>GAZ:00051993</oboInOwl:id>
        <rdfs:label>Deacon Peak</rdfs:label>
    </owl:NamedIndividual>
    


    <!-- http://purl.obolibrary.org/obo/GAZ_00051994 -->

    <owl:NamedIndividual rdf:about="http://purl.obolibrary.org/obo/GAZ_00051994">
        <obo:RO_0001025 rdf:resource="http://purl.obolibrary.org/obo/GAZ_00014121"/>
        <obo:IAO_0000115>A 7 km wide caldera flooded by the sea. Deception Island is located at the SW end of the Shetland Islands, NE of Graham Land Peninsula, and was constructed along the axis of the Bransfield Rift spreading center. A narrow passageway named Neptunes Bellows provides entrance to a natural harbor that was utilized as an Antarctic whaling station. Numerous vents located along ring fractures circling the low, 14 km wide island have been active during historical time. Maars line the shores of 190-m-deep Port Foster, the caldera bay. Among the largest of these maars is 1 km wide Whalers Bay, at the entrance to the harbor. Eruptions from Deception Island during the past 8700 years have been dated from ash layers in lake sediments on the Antarctic Peninsula and neighboring islands.</obo:IAO_0000115>
        <oboInOwl:hasOBONamespace>GAZ</oboInOwl:hasOBONamespace>
        <oboInOwl:id>GAZ:00051994</oboInOwl:id>
        <rdfs:label>Deception Island Caldera</rdfs:label>
    </owl:NamedIndividual>
    


    <!-- http://purl.obolibrary.org/obo/GAZ_00051998 -->

    <owl:NamedIndividual rdf:about="http://purl.obolibrary.org/obo/GAZ_00051998">
        <obo:RO_0001025 rdf:resource="http://purl.obolibrary.org/obo/GAZ_00045044"/>
        <obo:IAO_0000115>A youthful-looking shield volcano that forms an island along the Pacific Ocean coast of Antarctica&apos;s Marie Byrd Land. The massive 1800 cu km volcano is truncated by a 4-5 km summit caldera and is ringed by tuff cones at sea level. Its lack of dissection in a coastal area more susceptible to erosion than inland Antarctic volcanoes, and the existence of a satellite cone too young to date by the Potassium-Argon method, suggest a possible Holocene age (LeMasurier and Thomson 1990). The location of Mount Siple on published maps is 26 km NE of the actual location. A possible eruption cloud observed on satellite images on 1968-09-18 and 1988-10-04 was considered to result from atmospheric effects after low-level aerial observations revealed no evidence of recent eruptions (Smithsonian Scientific Event Alert Network Bulletin).</obo:IAO_0000115>
        <oboInOwl:hasOBONamespace>GAZ</oboInOwl:hasOBONamespace>
        <oboInOwl:id>GAZ:00051998</oboInOwl:id>
        <rdfs:label>Mount Siple</rdfs:label>
    </owl:NamedIndividual>
    


    <!-- http://purl.obolibrary.org/obo/GAZ_00052012 -->

    <owl:NamedIndividual rdf:about="http://purl.obolibrary.org/obo/GAZ_00052012">
        <obo:RO_0001025 rdf:resource="http://purl.obolibrary.org/obo/GAZ_00045015"/>
        <obo:IAO_0000115>A peak located at the northern end of Sturge Island. &quot;Volcanic activity&quot; was reported on a US Navy chart, but no indications of present or past activity were noted in 1959 (Catalog of Active Volcanoes of the World). No detailed geologic studies have been conducted in the inaccessible Balleny Islands.</obo:IAO_0000115>
        <oboInOwl:hasOBONamespace>GAZ</oboInOwl:hasOBONamespace>
        <oboInOwl:id>GAZ:00052012</oboInOwl:id>
        <rdfs:label>Russell Peak</rdfs:label>
    </owl:NamedIndividual>
    


    <!-- http://purl.obolibrary.org/obo/GAZ_00052013 -->

    <owl:NamedIndividual rdf:about="http://purl.obolibrary.org/obo/GAZ_00052013">
        <obo:RO_0001025 rdf:resource="http://purl.obolibrary.org/obo/GAZ_00045007"/>
        <obo:IAO_0000115>The initial report of a 12,000 foot volcano on Young Island proved incorrect--the island has a broad plateau-like summit reaching 1340 m. The island is almost completely mantled by ice.</obo:IAO_0000115>
        <oboInOwl:hasOBONamespace>GAZ</oboInOwl:hasOBONamespace>
        <oboInOwl:id>GAZ:00052013</oboInOwl:id>
        <rdfs:label>Freeman Peak</rdfs:label>
    </owl:NamedIndividual>
    


    <!-- http://purl.obolibrary.org/obo/GAZ_00053830 -->

    <owl:NamedIndividual rdf:about="http://purl.obolibrary.org/obo/GAZ_00053830">
        <rdf:type rdf:resource="http://purl.obolibrary.org/obo/ENVO_00000398"/>
        <obo:RO_0001025 rdf:resource="http://purl.obolibrary.org/obo/GAZ_00045014"/>
        <obo:IAO_0000115>A cone of the Buckle Island Volcano.</obo:IAO_0000115>
        <oboInOwl:hasOBONamespace>GAZ</oboInOwl:hasOBONamespace>
        <oboInOwl:id>GAZ:00053830</oboInOwl:id>
        <rdfs:label>Scott Cone</rdfs:label>
    </owl:NamedIndividual>
    


    <!-- http://purl.obolibrary.org/obo/GAZ_00053875 -->

    <owl:NamedIndividual rdf:about="http://purl.obolibrary.org/obo/GAZ_00053875">
        <obo:RO_0001025 rdf:resource="http://purl.obolibrary.org/obo/GAZ_00045015"/>
        <obo:IAO_0000115>The highest point of the Balleny Islands, on Sturge Island.</obo:IAO_0000115>
        <oboInOwl:hasOBONamespace>GAZ</oboInOwl:hasOBONamespace>
        <oboInOwl:id>GAZ:00053875</oboInOwl:id>
        <rdfs:label>Brown Peak</rdfs:label>
    </owl:NamedIndividual>
    


    <!-- http://purl.obolibrary.org/obo/GAZ_00058565 -->

    <owl:NamedIndividual rdf:about="http://purl.obolibrary.org/obo/GAZ_00058565">
        <obo:RO_0001025 rdf:resource="http://purl.obolibrary.org/obo/GAZ_00023316"/>
        <obo:IAO_0000115>A lake lying southeast of Skua Lake at Cape Evans, Ross Island.</obo:IAO_0000115>
        <oboInOwl:hasOBONamespace>GAZ</oboInOwl:hasOBONamespace>
        <oboInOwl:id>GAZ:00058565</oboInOwl:id>
        <rdfs:label>Island Lake</rdfs:label>
    </owl:NamedIndividual>
    


    <!-- http://purl.obolibrary.org/obo/GAZ_00058566 -->

    <owl:NamedIndividual rdf:about="http://purl.obolibrary.org/obo/GAZ_00058566">
        <obo:RO_0001025 rdf:resource="http://purl.obolibrary.org/obo/GAZ_00004057"/>
        <obo:IAO_0000115>A small lake close NW of Island Lake at Cape Evans, Ross Island.</obo:IAO_0000115>
        <oboInOwl:hasOBONamespace>GAZ</oboInOwl:hasOBONamespace>
        <oboInOwl:id>GAZ:00058566</oboInOwl:id>
        <rdfs:label>Skua Lake</rdfs:label>
    </owl:NamedIndividual>
    


    <!-- http://purl.obolibrary.org/obo/GAZ_00058568 -->

    <owl:NamedIndividual rdf:about="http://purl.obolibrary.org/obo/GAZ_00058568">
        <obo:RO_0001025 rdf:resource="http://purl.obolibrary.org/obo/GAZ_00023334"/>
        <obo:IAO_0000115>A lake 0.4 km NW of Jasper Point in northeast Fildes Peninsula, King George Island.</obo:IAO_0000115>
        <oboInOwl:hasOBONamespace>GAZ</oboInOwl:hasOBONamespace>
        <oboInOwl:id>GAZ:00058568</oboInOwl:id>
        <rdfs:label>Lake Profound</rdfs:label>
    </owl:NamedIndividual>
    


    <!-- http://purl.obolibrary.org/obo/GAZ_00058569 -->

    <owl:NamedIndividual rdf:about="http://purl.obolibrary.org/obo/GAZ_00058569">
        <obo:RO_0001025 rdf:resource="http://purl.obolibrary.org/obo/GAZ_00007329"/>
        <obo:IAO_0000115>A ridge rising to 161 m in Eastern Livingston Island, Antarctica. To the west the ridge surmounts the South Bay coast north of Johnsons Dock, to the south it is bounded by the lower course of the two km long Contell Glacier, to the east by the foot of the Balkan Snowfield sloping up towards Krum Rock and to the northwest by Sea Lion Tarn.</obo:IAO_0000115>
        <oboInOwl:hasOBONamespace>GAZ</oboInOwl:hasOBONamespace>
        <oboInOwl:id>GAZ:00058569</oboInOwl:id>
        <rdfs:label>Atlantic Club Ridge</rdfs:label>
    </owl:NamedIndividual>
    


    <!-- http://purl.obolibrary.org/obo/GAZ_00058570 -->

    <owl:NamedIndividual rdf:about="http://purl.obolibrary.org/obo/GAZ_00058570">
        <obo:RO_0001025 rdf:resource="http://purl.obolibrary.org/obo/GAZ_00058569"/>
        <obo:IAO_0000115>A 0.3 ha tarn located between Sea Lion Glacier and the north-western slopes of Atlantic Club Ridge in eastern Livingston Island, Antarctica.</obo:IAO_0000115>
        <oboInOwl:hasOBONamespace>GAZ</oboInOwl:hasOBONamespace>
        <oboInOwl:id>GAZ:00058570</oboInOwl:id>
        <rdfs:label>Sea Lion Tarn</rdfs:label>
    </owl:NamedIndividual>
    


    <!-- http://purl.obolibrary.org/obo/GAZ_00129075 -->

    <owl:NamedIndividual rdf:about="http://purl.obolibrary.org/obo/GAZ_00129075">
        <obo:RO_0001025 rdf:resource="http://purl.obolibrary.org/obo/GAZ_00009523"/>
        <obo:IAO_0000115>An insular rock, 165 m high, lying 0.9 km northwest of Route Point, the northwest tip of Laurie Island in the South Orkney Islands. It is between the Mackenzie Peninsula and Eillium Island.</obo:IAO_0000115>
        <oboInOwl:hasOBONamespace>GAZ</oboInOwl:hasOBONamespace>
        <oboInOwl:id>GAZ:00129075</oboInOwl:id>
        <rdfs:label>Nigg Rock</rdfs:label>
    </owl:NamedIndividual>
    


    <!-- http://purl.obolibrary.org/obo/GAZ_00129076 -->

    <owl:NamedIndividual rdf:about="http://purl.obolibrary.org/obo/GAZ_00129076">
        <obo:RO_0001025 rdf:resource="http://purl.obolibrary.org/obo/GAZ_00007328"/>
        <obo:IAO_0000115>One of the minor islands in the South Shetlands archipelago, Antarctica, which is situated off the north coast of Livingston Island.</obo:IAO_0000115>
        <oboInOwl:hasOBONamespace>GAZ</oboInOwl:hasOBONamespace>
        <oboInOwl:id>GAZ:00129076</oboInOwl:id>
        <rdfs:label>Desolation Island</rdfs:label>
    </owl:NamedIndividual>
    


    <!-- http://purl.obolibrary.org/obo/GAZ_00129077 -->

    <owl:NamedIndividual rdf:about="http://purl.obolibrary.org/obo/GAZ_00129077">
        <obo:RO_0001025 rdf:resource="http://purl.obolibrary.org/obo/GAZ_00023318"/>
        <obo:IAO_0000115>An Argentine base in Antarctica, and the first permanent base in the area defined by the Antarctic Treaty System. It is located on Laurie Island, one of the South Orkney Islands. Established 1904.</obo:IAO_0000115>
        <oboInOwl:hasOBONamespace>GAZ</oboInOwl:hasOBONamespace>
        <oboInOwl:id>GAZ:00129077</oboInOwl:id>
        <rdfs:label>Orcadas Base</rdfs:label>
    </owl:NamedIndividual>
    


    <!-- http://purl.obolibrary.org/obo/GAZ_00136629 -->

    <owl:NamedIndividual rdf:about="http://purl.obolibrary.org/obo/GAZ_00136629">
        <obo:RO_0001025 rdf:resource="http://purl.obolibrary.org/obo/GAZ_00023334"/>
        <obo:IAO_0000115>The most important Antarctic base of Chile. It is located at Fildes Peninsula, an ice-free area, in front of Fildes Bay (Maxwell Bay), west of King George Island, South Shetland Islands.</obo:IAO_0000115>
        <oboInOwl:hasOBONamespace>GAZ</oboInOwl:hasOBONamespace>
        <oboInOwl:id>GAZ:00136629</oboInOwl:id>
        <rdfs:label>Base Presidente Eduardo Frei Montalva</rdfs:label>
    </owl:NamedIndividual>
    


    <!-- http://purl.obolibrary.org/obo/GAZ_00136630 -->

    <owl:NamedIndividual rdf:about="http://purl.obolibrary.org/obo/GAZ_00136630">
        <obo:RO_0001025 rdf:resource="http://purl.obolibrary.org/obo/GAZ_00023334"/>
        <obo:IAO_0000115>A permanent Chilean Antarctic research base. It is located on King George Island. It lies within the Antartica Chilean commune.</obo:IAO_0000115>
        <oboInOwl:hasOBONamespace>GAZ</oboInOwl:hasOBONamespace>
        <oboInOwl:id>GAZ:00136630</oboInOwl:id>
        <rdfs:label>Professor Julio Escudero Base</rdfs:label>
    </owl:NamedIndividual>
    


    <!-- http://purl.obolibrary.org/obo/GAZ_00136632 -->

    <owl:NamedIndividual rdf:about="http://purl.obolibrary.org/obo/GAZ_00136632">
        <obo:RO_0001025 rdf:resource="http://purl.obolibrary.org/obo/GAZ_00140059"/>
        <obo:IAO_0000115>A harbor in King George Island in Antarctica. It is mainly a Russian owned area with their Bellinghausen Station on the coast.</obo:IAO_0000115>
        <oboInOwl:hasOBONamespace>GAZ</oboInOwl:hasOBONamespace>
        <oboInOwl:id>GAZ:00136632</oboInOwl:id>
        <rdfs:label>Collins Harbour</rdfs:label>
    </owl:NamedIndividual>
    


    <!-- http://purl.obolibrary.org/obo/GAZ_00136633 -->

    <owl:NamedIndividual rdf:about="http://purl.obolibrary.org/obo/GAZ_00136633">
        <obo:RO_0001025 rdf:resource="http://purl.obolibrary.org/obo/GAZ_00136629"/>
        <obo:IAO_0000115>A Chilean hamlet in Antartica Commune, Antartica Province, Magallanes and Antartica Chilena Region. It is located in the Chilean Antarctic base of Frei Montalva, in King George Island.</obo:IAO_0000115>
        <oboInOwl:hasOBONamespace>GAZ</oboInOwl:hasOBONamespace>
        <oboInOwl:id>GAZ:00136633</oboInOwl:id>
        <rdfs:label>Villa Las Estrellas</rdfs:label>
    </owl:NamedIndividual>
    


    <!-- http://purl.obolibrary.org/obo/GAZ_00136641 -->

    <owl:NamedIndividual rdf:about="http://purl.obolibrary.org/obo/GAZ_00136641">
        <obo:RO_0001025 rdf:resource="http://purl.obolibrary.org/obo/GAZ_00007328"/>
        <obo:IAO_0000115>A small island 6 km west of Gibbs Island in the South Shetland Islands.</obo:IAO_0000115>
        <oboInOwl:hasOBONamespace>GAZ</oboInOwl:hasOBONamespace>
        <oboInOwl:id>GAZ:00136641</oboInOwl:id>
        <rdfs:label>Aspland Island</rdfs:label>
    </owl:NamedIndividual>
    


    <!-- http://purl.obolibrary.org/obo/GAZ_00139118 -->

    <owl:NamedIndividual rdf:about="http://purl.obolibrary.org/obo/GAZ_00139118">
        <obo:RO_0001025 rdf:resource="http://purl.obolibrary.org/obo/GAZ_00014088"/>
        <obo:IAO_0000115>An oasis area on the E coast of Ablation Island, facing George VI Sound.</obo:IAO_0000115>
        <oboInOwl:hasOBONamespace>GAZ</oboInOwl:hasOBONamespace>
        <oboInOwl:id>GAZ:00139118</oboInOwl:id>
        <rdfs:label>Ablation Point</rdfs:label>
    </owl:NamedIndividual>
    


    <!-- http://purl.obolibrary.org/obo/GAZ_00139119 -->

    <owl:NamedIndividual rdf:about="http://purl.obolibrary.org/obo/GAZ_00139119">
        <obo:RO_0001025 rdf:resource="http://purl.obolibrary.org/obo/GAZ_00014088"/>
        <obo:IAO_0000115>A relatively ice-free valley on the E coast of Alexander Island.</obo:IAO_0000115>
        <oboInOwl:hasOBONamespace>GAZ</oboInOwl:hasOBONamespace>
        <oboInOwl:id>GAZ:00139119</oboInOwl:id>
        <rdfs:label>Ablation Valley</rdfs:label>
    </owl:NamedIndividual>
    


    <!-- http://purl.obolibrary.org/obo/GAZ_00139123 -->

    <owl:NamedIndividual rdf:about="http://purl.obolibrary.org/obo/GAZ_00139123">
        <obo:RO_0001025 rdf:resource="http://purl.obolibrary.org/obo/GAZ_00023301"/>
        <obo:IAO_0000115>A former (1961-1977) British research station on the SW corner of Adelaide Island.</obo:IAO_0000115>
        <oboInOwl:hasOBONamespace>GAZ</oboInOwl:hasOBONamespace>
        <oboInOwl:id>GAZ:00139123</oboInOwl:id>
        <rdfs:label>Adelaide</rdfs:label>
    </owl:NamedIndividual>
    


    <!-- http://purl.obolibrary.org/obo/GAZ_00139124 -->

    <owl:NamedIndividual rdf:about="http://purl.obolibrary.org/obo/GAZ_00139124">
        <obo:RO_0001025 rdf:resource="http://purl.obolibrary.org/obo/GAZ_00007426"/>
        <obo:IAO_0000115>An inlet of Admirality Bay.</obo:IAO_0000115>
        <oboInOwl:hasOBONamespace>GAZ</oboInOwl:hasOBONamespace>
        <oboInOwl:id>GAZ:00139124</oboInOwl:id>
        <rdfs:label>Mackellar Inlet</rdfs:label>
    </owl:NamedIndividual>
    


    <!-- http://purl.obolibrary.org/obo/GAZ_00139125 -->

    <owl:NamedIndividual rdf:about="http://purl.obolibrary.org/obo/GAZ_00139125">
        <obo:RO_0001025 rdf:resource="http://purl.obolibrary.org/obo/GAZ_00007426"/>
        <obo:IAO_0000115>An inlet of Admirality Bay.</obo:IAO_0000115>
        <oboInOwl:hasOBONamespace>GAZ</oboInOwl:hasOBONamespace>
        <oboInOwl:id>GAZ:00139125</oboInOwl:id>
        <rdfs:label>Martel Inlet</rdfs:label>
    </owl:NamedIndividual>
    


    <!-- http://purl.obolibrary.org/obo/GAZ_00139126 -->

    <owl:NamedIndividual rdf:about="http://purl.obolibrary.org/obo/GAZ_00139126">
        <obo:RO_0001025 rdf:resource="http://purl.obolibrary.org/obo/GAZ_00007426"/>
        <obo:IAO_0000115>An inlet of Admirality Bay.</obo:IAO_0000115>
        <oboInOwl:hasOBONamespace>GAZ</oboInOwl:hasOBONamespace>
        <oboInOwl:id>GAZ:00139126</oboInOwl:id>
        <rdfs:label>Escurra Inlet</rdfs:label>
    </owl:NamedIndividual>
    


    <!-- http://purl.obolibrary.org/obo/GAZ_00139127 -->

    <owl:NamedIndividual rdf:about="http://purl.obolibrary.org/obo/GAZ_00139127">
        <obo:RO_0001025 rdf:resource="http://purl.obolibrary.org/obo/GAZ_00139126"/>
        <obo:IAO_0000115>An island in Escurra Inlet.</obo:IAO_0000115>
        <oboInOwl:hasOBONamespace>GAZ</oboInOwl:hasOBONamespace>
        <oboInOwl:id>GAZ:00139127</oboInOwl:id>
        <rdfs:label>Dufayal Island</rdfs:label>
    </owl:NamedIndividual>
    


    <!-- http://purl.obolibrary.org/obo/GAZ_00139129 -->

    <owl:NamedIndividual rdf:about="http://purl.obolibrary.org/obo/GAZ_00139129">
        <obo:RO_0001025 rdf:resource="http://purl.obolibrary.org/obo/GAZ_00014123"/>
        <oboInOwl:hasOBONamespace>GAZ</oboInOwl:hasOBONamespace>
        <oboInOwl:id>GAZ:00139129</oboInOwl:id>
        <rdfs:label>Marina Point</rdfs:label>
    </owl:NamedIndividual>
    


    <!-- http://purl.obolibrary.org/obo/GAZ_00139130 -->

    <owl:NamedIndividual rdf:about="http://purl.obolibrary.org/obo/GAZ_00139130">
        <obo:RO_0001025 rdf:resource="http://purl.obolibrary.org/obo/GAZ_00139129"/>
        <obo:IAO_0000115>A year-round Ukrainian research station. Formerly a British research station. Established 1994.</obo:IAO_0000115>
        <oboInOwl:hasOBONamespace>GAZ</oboInOwl:hasOBONamespace>
        <oboInOwl:id>GAZ:00139130</oboInOwl:id>
        <rdfs:label>Akademik Vernadsky Station</rdfs:label>
    </owl:NamedIndividual>
    


    <!-- http://purl.obolibrary.org/obo/GAZ_00139133 -->

    <owl:NamedIndividual rdf:about="http://purl.obolibrary.org/obo/GAZ_00139133">
        <rdf:type rdf:resource="http://purl.obolibrary.org/obo/ENVO_00000305"/>
        <obo:RO_0001025 rdf:resource="http://purl.obolibrary.org/obo/GAZ_00023301"/>
        <obo:IAO_0000115>A cape on the SW corner of Adelaide Island.</obo:IAO_0000115>
        <oboInOwl:hasOBONamespace>GAZ</oboInOwl:hasOBONamespace>
        <oboInOwl:id>GAZ:00139133</oboInOwl:id>
        <rdfs:label>Cape Alexandra</rdfs:label>
    </owl:NamedIndividual>
    


    <!-- http://purl.obolibrary.org/obo/GAZ_00139140 -->

    <owl:NamedIndividual rdf:about="http://purl.obolibrary.org/obo/GAZ_00139140">
        <obo:RO_0001025 rdf:resource="http://purl.obolibrary.org/obo/GAZ_00004047"/>
        <obo:IAO_0000115>A wide embayment behind Lemaire and Bryde Islands, indenting the W coast of Graham Land between Duthiers and Leniz Points.</obo:IAO_0000115>
        <oboInOwl:hasOBONamespace>GAZ</oboInOwl:hasOBONamespace>
        <oboInOwl:id>GAZ:00139140</oboInOwl:id>
        <rdfs:label>Paradise Bay</rdfs:label>
    </owl:NamedIndividual>
    


    <!-- http://purl.obolibrary.org/obo/GAZ_00139141 -->

    <owl:NamedIndividual rdf:about="http://purl.obolibrary.org/obo/GAZ_00139141">
        <rdf:type rdf:resource="http://purl.obolibrary.org/obo/ENVO_00000305"/>
        <obo:RO_0001025 rdf:resource="http://purl.obolibrary.org/obo/GAZ_00023319"/>
        <obo:IAO_0000115>A headland on the S coast of Coronation Island.</obo:IAO_0000115>
        <oboInOwl:hasOBONamespace>GAZ</oboInOwl:hasOBONamespace>
        <oboInOwl:id>GAZ:00139141</oboInOwl:id>
        <rdfs:label>Amphibolite Point</rdfs:label>
    </owl:NamedIndividual>
    


    <!-- http://purl.obolibrary.org/obo/GAZ_00139144 -->

    <owl:NamedIndividual rdf:about="http://purl.obolibrary.org/obo/GAZ_00139144">
        <obo:RO_0001025 rdf:resource="http://purl.obolibrary.org/obo/GAZ_00051527"/>
        <obo:IAO_0000115>An island, 1.5 mi long, which lies immediately N of Omega Island in the Melchior Islands, Palmer Archipelago.</obo:IAO_0000115>
        <oboInOwl:hasOBONamespace>GAZ</oboInOwl:hasOBONamespace>
        <oboInOwl:id>GAZ:00139144</oboInOwl:id>
        <rdfs:label>Eta Island</rdfs:label>
    </owl:NamedIndividual>
    


    <!-- http://purl.obolibrary.org/obo/GAZ_00139145 -->

    <owl:NamedIndividual rdf:about="http://purl.obolibrary.org/obo/GAZ_00139145">
        <obo:RO_0001025 rdf:resource="http://purl.obolibrary.org/obo/GAZ_00051527"/>
        <obo:IAO_0000115>An island 2 mi long, which lies immediately S of Eta Island in the Melchior Islands, Palmer Archipelago.</obo:IAO_0000115>
        <oboInOwl:hasOBONamespace>GAZ</oboInOwl:hasOBONamespace>
        <oboInOwl:id>GAZ:00139145</oboInOwl:id>
        <rdfs:label>Omega Island</rdfs:label>
    </owl:NamedIndividual>
    


    <!-- http://purl.obolibrary.org/obo/GAZ_00139146 -->

    <owl:NamedIndividual rdf:about="http://purl.obolibrary.org/obo/GAZ_00139146">
        <obo:RO_0001025 rdf:resource="http://purl.obolibrary.org/obo/GAZ_00051528"/>
        <obo:IAO_0000115>A harbour between Eta and Omega Islands.</obo:IAO_0000115>
        <oboInOwl:hasOBONamespace>GAZ</oboInOwl:hasOBONamespace>
        <oboInOwl:id>GAZ:00139146</oboInOwl:id>
        <rdfs:label>Anderson Harbour</rdfs:label>
    </owl:NamedIndividual>
    


    <!-- http://purl.obolibrary.org/obo/GAZ_00139149 -->

    <owl:NamedIndividual rdf:about="http://purl.obolibrary.org/obo/GAZ_00139149">
        <obo:RO_0001025 rdf:resource="http://purl.obolibrary.org/obo/GAZ_00141552"/>
        <obo:IAO_0000115>A glacier-lined bay on the SW side of the Arctowski Peninsula.</obo:IAO_0000115>
        <oboInOwl:hasOBONamespace>GAZ</oboInOwl:hasOBONamespace>
        <oboInOwl:id>GAZ:00139149</oboInOwl:id>
        <rdfs:label>Andvord Bay</rdfs:label>
    </owl:NamedIndividual>
    


    <!-- http://purl.obolibrary.org/obo/GAZ_00139150 -->

    <owl:NamedIndividual rdf:about="http://purl.obolibrary.org/obo/GAZ_00139150">
        <obo:RO_0001025 rdf:resource="http://purl.obolibrary.org/obo/GAZ_00004045"/>
        <obo:IAO_0000115>A channel between D&apos;Urville Island and Trinity Peninsula.</obo:IAO_0000115>
        <oboInOwl:hasOBONamespace>GAZ</oboInOwl:hasOBONamespace>
        <oboInOwl:id>GAZ:00139150</oboInOwl:id>
        <rdfs:label>Antarctic Sound</rdfs:label>
    </owl:NamedIndividual>
    


    <!-- http://purl.obolibrary.org/obo/GAZ_00139151 -->

    <owl:NamedIndividual rdf:about="http://purl.obolibrary.org/obo/GAZ_00139151">
        <obo:RO_0001025 rdf:resource="http://purl.obolibrary.org/obo/GAZ_00004381"/>
        <obo:IAO_0000115>A former UK base in Arthur Harbor.</obo:IAO_0000115>
        <oboInOwl:hasOBONamespace>GAZ</oboInOwl:hasOBONamespace>
        <oboInOwl:id>GAZ:00139151</oboInOwl:id>
        <rdfs:label>Base N</rdfs:label>
    </owl:NamedIndividual>
    


    <!-- http://purl.obolibrary.org/obo/GAZ_00139155 -->

    <owl:NamedIndividual rdf:about="http://purl.obolibrary.org/obo/GAZ_00139155">
        <obo:RO_0001025 rdf:resource="http://purl.obolibrary.org/obo/GAZ_00004057"/>
        <obo:IAO_0000115>Heights overlooking Hut Point.</obo:IAO_0000115>
        <oboInOwl:hasOBONamespace>GAZ</oboInOwl:hasOBONamespace>
        <oboInOwl:id>GAZ:00139155</oboInOwl:id>
        <rdfs:label>Arrival Heights</rdfs:label>
    </owl:NamedIndividual>
    


    <!-- http://purl.obolibrary.org/obo/GAZ_00139157 -->

    <owl:NamedIndividual rdf:about="http://purl.obolibrary.org/obo/GAZ_00139157">
        <obo:RO_0001025 rdf:resource="http://purl.obolibrary.org/obo/GAZ_00141552"/>
        <obo:IAO_0000115>A harbor between Bonaparte Point and Norsel Point, on the SE coast of Anvers Island.</obo:IAO_0000115>
        <oboInOwl:hasOBONamespace>GAZ</oboInOwl:hasOBONamespace>
        <oboInOwl:id>GAZ:00139157</oboInOwl:id>
        <rdfs:label>Arthur Harbour</rdfs:label>
    </owl:NamedIndividual>
    


    <!-- http://purl.obolibrary.org/obo/GAZ_00139158 -->

    <owl:NamedIndividual rdf:about="http://purl.obolibrary.org/obo/GAZ_00139158">
        <obo:RO_0001025 rdf:resource="http://purl.obolibrary.org/obo/GAZ_00004381"/>
        <obo:IAO_0000115>A rocky point on the northwest side of Arthur Harbor, on the southwest coast of Anvers Island in the Palmer Archipelago.</obo:IAO_0000115>
        <oboInOwl:hasOBONamespace>GAZ</oboInOwl:hasOBONamespace>
        <oboInOwl:id>GAZ:00139158</oboInOwl:id>
        <rdfs:label>Norsel Point</rdfs:label>
    </owl:NamedIndividual>
    


    <!-- http://purl.obolibrary.org/obo/GAZ_00139159 -->

    <owl:NamedIndividual rdf:about="http://purl.obolibrary.org/obo/GAZ_00139159">
        <rdf:type rdf:resource="http://purl.obolibrary.org/obo/ENVO_00000167"/>
        <obo:RO_0001025 rdf:resource="http://purl.obolibrary.org/obo/GAZ_00004381"/>
        <obo:IAO_0000115>A narrow point at the south side of Arthur Harbor on the southwest coast of Anvers Island, in the Palmer Archipelago.</obo:IAO_0000115>
        <oboInOwl:hasOBONamespace>GAZ</oboInOwl:hasOBONamespace>
        <oboInOwl:id>GAZ:00139159</oboInOwl:id>
        <rdfs:label>Bonaparte Point</rdfs:label>
    </owl:NamedIndividual>
    


    <!-- http://purl.obolibrary.org/obo/GAZ_00139160 -->

    <owl:NamedIndividual rdf:about="http://purl.obolibrary.org/obo/GAZ_00139160">
        <obo:RO_0001025 rdf:resource="http://purl.obolibrary.org/obo/GAZ_00023334"/>
        <obo:IAO_0000115>A Uruguayan research station near Lake Profound.</obo:IAO_0000115>
        <oboInOwl:hasOBONamespace>GAZ</oboInOwl:hasOBONamespace>
        <oboInOwl:id>GAZ:00139160</oboInOwl:id>
        <rdfs:label>Artigas Station</rdfs:label>
    </owl:NamedIndividual>
    


    <!-- http://purl.obolibrary.org/obo/GAZ_00139164 -->

    <owl:NamedIndividual rdf:about="http://purl.obolibrary.org/obo/GAZ_00139164">
        <obo:RO_0001025 rdf:resource="http://purl.obolibrary.org/obo/GAZ_00014089"/>
        <obo:IAO_0000115>An island off the SW tip of Adelaide Island.</obo:IAO_0000115>
        <oboInOwl:hasOBONamespace>GAZ</oboInOwl:hasOBONamespace>
        <oboInOwl:id>GAZ:00139164</oboInOwl:id>
        <rdfs:label>Avian Island</rdfs:label>
    </owl:NamedIndividual>
    


    <!-- http://purl.obolibrary.org/obo/GAZ_00139195 -->

    <owl:NamedIndividual rdf:about="http://purl.obolibrary.org/obo/GAZ_00139195">
        <obo:RO_0001025 rdf:resource="http://purl.obolibrary.org/obo/GAZ_00014084"/>
        <obo:IAO_0000115>An ice shelf occupying a large bay on the southern end of Alexander Island.</obo:IAO_0000115>
        <oboInOwl:hasOBONamespace>GAZ</oboInOwl:hasOBONamespace>
        <oboInOwl:id>GAZ:00139195</oboInOwl:id>
        <rdfs:label>Bach Ice Shelf</rdfs:label>
    </owl:NamedIndividual>
    


    <!-- http://purl.obolibrary.org/obo/GAZ_00139197 -->

    <owl:NamedIndividual rdf:about="http://purl.obolibrary.org/obo/GAZ_00139197">
        <obo:RO_0001025 rdf:resource="http://purl.obolibrary.org/obo/GAZ_00004045"/>
        <obo:IAO_0000115>An ice shelf off the Banzare Coast.</obo:IAO_0000115>
        <oboInOwl:hasOBONamespace>GAZ</oboInOwl:hasOBONamespace>
        <oboInOwl:id>GAZ:00139197</oboInOwl:id>
        <rdfs:label>Voyeykov Ice Shelf</rdfs:label>
    </owl:NamedIndividual>
    


    <!-- http://purl.obolibrary.org/obo/GAZ_00139204 -->

    <owl:NamedIndividual rdf:about="http://purl.obolibrary.org/obo/GAZ_00139204">
        <obo:RO_0001025 rdf:resource="http://purl.obolibrary.org/obo/GAZ_00023334"/>
        <obo:IAO_0000115>Russian (formerly Soviet) Antarctic station at Collins Harbour, on King George Island of the South Shetland Islands.</obo:IAO_0000115>
        <oboInOwl:hasOBONamespace>GAZ</oboInOwl:hasOBONamespace>
        <oboInOwl:id>GAZ:00139204</oboInOwl:id>
        <rdfs:label>Bellingshausen Station</rdfs:label>
    </owl:NamedIndividual>
    


    <!-- http://purl.obolibrary.org/obo/GAZ_00139205 -->

    <owl:NamedIndividual rdf:about="http://purl.obolibrary.org/obo/GAZ_00139205">
        <obo:RO_0001025 rdf:resource="http://purl.obolibrary.org/obo/GAZ_00141552"/>
        <obo:IAO_0000115>A fjord between Pourquoi Pas Island and the Arrowsmith Peninsula.</obo:IAO_0000115>
        <oboInOwl:hasOBONamespace>GAZ</oboInOwl:hasOBONamespace>
        <oboInOwl:id>GAZ:00139205</oboInOwl:id>
        <rdfs:label>Bigourdan Fjord</rdfs:label>
    </owl:NamedIndividual>
    


    <!-- http://purl.obolibrary.org/obo/GAZ_00139208 -->

    <owl:NamedIndividual rdf:about="http://purl.obolibrary.org/obo/GAZ_00139208">
        <obo:RO_0001025 rdf:resource="http://purl.obolibrary.org/obo/GAZ_00004381"/>
        <obo:IAO_0000115>A rocky promontory on the SE side of Biscoe Bay.</obo:IAO_0000115>
        <oboInOwl:hasOBONamespace>GAZ</oboInOwl:hasOBONamespace>
        <oboInOwl:id>GAZ:00139208</oboInOwl:id>
        <rdfs:label>Biscoe Point</rdfs:label>
    </owl:NamedIndividual>
    


    <!-- http://purl.obolibrary.org/obo/GAZ_00139209 -->

    <owl:NamedIndividual rdf:about="http://purl.obolibrary.org/obo/GAZ_00139209">
        <obo:RO_0001025 rdf:resource="http://purl.obolibrary.org/obo/GAZ_00141552"/>
        <obo:IAO_0000115>A bay which indents the SW coast of Anvers Island immediately N of Biscoe Point, in the Palmer Archipelago, Antarctica.</obo:IAO_0000115>
        <oboInOwl:hasOBONamespace>GAZ</oboInOwl:hasOBONamespace>
        <oboInOwl:id>GAZ:00139209</oboInOwl:id>
        <rdfs:label>Biscoe Bay</rdfs:label>
    </owl:NamedIndividual>
    


    <!-- http://purl.obolibrary.org/obo/GAZ_00139210 -->

    <owl:NamedIndividual rdf:about="http://purl.obolibrary.org/obo/GAZ_00139210">
        <obo:RO_0001025 rdf:resource="http://purl.obolibrary.org/obo/GAZ_00141552"/>
        <obo:IAO_0000115>A straight between S Anvers Island and Wiencke Island and Wauwermans Islands.</obo:IAO_0000115>
        <oboInOwl:hasOBONamespace>GAZ</oboInOwl:hasOBONamespace>
        <oboInOwl:id>GAZ:00139210</oboInOwl:id>
        <rdfs:label>Bismark Strait</rdfs:label>
    </owl:NamedIndividual>
    


    <!-- http://purl.obolibrary.org/obo/GAZ_00139211 -->

    <owl:NamedIndividual rdf:about="http://purl.obolibrary.org/obo/GAZ_00139211">
        <obo:RO_0001025 rdf:resource="http://purl.obolibrary.org/obo/GAZ_00014089"/>
        <obo:IAO_0000115>An island separating Bigourdan and Bourgeois Fjords.</obo:IAO_0000115>
        <oboInOwl:hasOBONamespace>GAZ</oboInOwl:hasOBONamespace>
        <oboInOwl:id>GAZ:00139211</oboInOwl:id>
        <rdfs:label>Blaiklock Island</rdfs:label>
    </owl:NamedIndividual>
    


    <!-- http://purl.obolibrary.org/obo/GAZ_00139216 -->

    <owl:NamedIndividual rdf:about="http://purl.obolibrary.org/obo/GAZ_00139216">
        <obo:RO_0001025 rdf:resource="http://purl.obolibrary.org/obo/GAZ_00014089"/>
        <obo:IAO_0000115>A fjord between Pourquoi Pas Island and the main Fallieres Coast, opening into northern Marguerite Bay.</obo:IAO_0000115>
        <oboInOwl:hasOBONamespace>GAZ</oboInOwl:hasOBONamespace>
        <oboInOwl:id>GAZ:00139216</oboInOwl:id>
        <rdfs:label>Bourgeois Fjord</rdfs:label>
    </owl:NamedIndividual>
    


    <!-- http://purl.obolibrary.org/obo/GAZ_00139221 -->

    <owl:NamedIndividual rdf:about="http://purl.obolibrary.org/obo/GAZ_00139221">
        <obo:RO_0001025 rdf:resource="http://purl.obolibrary.org/obo/GAZ_00051133"/>
        <obo:IAO_0000115>An island off the Bowman Coast.</obo:IAO_0000115>
        <oboInOwl:hasOBONamespace>GAZ</oboInOwl:hasOBONamespace>
        <oboInOwl:id>GAZ:00139221</oboInOwl:id>
        <rdfs:label>Francis Island</rdfs:label>
    </owl:NamedIndividual>
    


    <!-- http://purl.obolibrary.org/obo/GAZ_00139222 -->

    <owl:NamedIndividual rdf:about="http://purl.obolibrary.org/obo/GAZ_00139222">
        <obo:RO_0001025 rdf:resource="http://purl.obolibrary.org/obo/GAZ_00140059"/>
        <obo:IAO_0000115>A strait separating Snow Island and Smith Island in the W of the South Sheltland Islands.</obo:IAO_0000115>
        <oboInOwl:hasOBONamespace>GAZ</oboInOwl:hasOBONamespace>
        <oboInOwl:id>GAZ:00139222</oboInOwl:id>
        <rdfs:label>Boyd Strait</rdfs:label>
    </owl:NamedIndividual>
    


    <!-- http://purl.obolibrary.org/obo/GAZ_00139225 -->

    <owl:NamedIndividual rdf:about="http://purl.obolibrary.org/obo/GAZ_00139225">
        <obo:RO_0001025 rdf:resource="http://purl.obolibrary.org/obo/GAZ_00004045"/>
        <obo:IAO_0000115>An ice shelf bordering the Caird Coast, between Dawson-Lambton Glacier and Stancomb-Wills Glacier Tongue.</obo:IAO_0000115>
        <oboInOwl:hasOBONamespace>GAZ</oboInOwl:hasOBONamespace>
        <oboInOwl:id>GAZ:00139225</oboInOwl:id>
        <rdfs:label>Brunt Ice Shelf</rdfs:label>
    </owl:NamedIndividual>
    


    <!-- http://purl.obolibrary.org/obo/GAZ_00139396 -->

    <owl:NamedIndividual rdf:about="http://purl.obolibrary.org/obo/GAZ_00139396">
        <obo:RO_0001025 rdf:resource="http://purl.obolibrary.org/obo/GAZ_00023318"/>
        <oboInOwl:hasOBONamespace>GAZ</oboInOwl:hasOBONamespace>
        <oboInOwl:id>GAZ:00139396</oboInOwl:id>
        <rdfs:label>Ferguslike Peninsula</rdfs:label>
    </owl:NamedIndividual>
    


    <!-- http://purl.obolibrary.org/obo/GAZ_00139397 -->

    <owl:NamedIndividual rdf:about="http://purl.obolibrary.org/obo/GAZ_00139397">
        <obo:RO_0001025 rdf:resource="http://purl.obolibrary.org/obo/GAZ_00139396"/>
        <obo:IAO_0000115>A former British research base (1946-1947).</obo:IAO_0000115>
        <oboInOwl:hasOBONamespace>GAZ</oboInOwl:hasOBONamespace>
        <oboInOwl:id>GAZ:00139397</oboInOwl:id>
        <rdfs:label>Cape Geddes Base</rdfs:label>
    </owl:NamedIndividual>
    


    <!-- http://purl.obolibrary.org/obo/GAZ_00139398 -->

    <owl:NamedIndividual rdf:about="http://purl.obolibrary.org/obo/GAZ_00139398">
        <obo:RO_0001025 rdf:resource="http://purl.obolibrary.org/obo/GAZ_00017735"/>
        <obo:IAO_0000115>A peninsula within Discovery Bay on the N coast of Greenwich Island.</obo:IAO_0000115>
        <oboInOwl:hasOBONamespace>GAZ</oboInOwl:hasOBONamespace>
        <oboInOwl:id>GAZ:00139398</oboInOwl:id>
        <rdfs:label>Guesalaga Peninsula</rdfs:label>
    </owl:NamedIndividual>
    


    <!-- http://purl.obolibrary.org/obo/GAZ_00139399 -->

    <owl:NamedIndividual rdf:about="http://purl.obolibrary.org/obo/GAZ_00139399">
        <obo:RO_0001025 rdf:resource="http://purl.obolibrary.org/obo/GAZ_00139398"/>
        <obo:IAO_0000115>A Chilean naval station. Established 1947.</obo:IAO_0000115>
        <oboInOwl:hasOBONamespace>GAZ</oboInOwl:hasOBONamespace>
        <oboInOwl:id>GAZ:00139399</oboInOwl:id>
        <rdfs:label>Capitan Arturo Prat Station</rdfs:label>
    </owl:NamedIndividual>
    


    <!-- http://purl.obolibrary.org/obo/GAZ_00139400 -->

    <owl:NamedIndividual rdf:about="http://purl.obolibrary.org/obo/GAZ_00139400">
        <obo:RO_0001025 rdf:resource="http://purl.obolibrary.org/obo/GAZ_00004057"/>
        <obo:IAO_0000115>A beach 1 km N of Cape Bird.</obo:IAO_0000115>
        <oboInOwl:hasOBONamespace>GAZ</oboInOwl:hasOBONamespace>
        <oboInOwl:id>GAZ:00139400</oboInOwl:id>
        <rdfs:label>Caughley Beach</rdfs:label>
    </owl:NamedIndividual>
    


    <!-- http://purl.obolibrary.org/obo/GAZ_00139401 -->

    <owl:NamedIndividual rdf:about="http://purl.obolibrary.org/obo/GAZ_00139401">
        <obo:RO_0001025 rdf:resource="http://purl.obolibrary.org/obo/GAZ_00004057"/>
        <oboInOwl:hasOBONamespace>GAZ</oboInOwl:hasOBONamespace>
        <oboInOwl:id>GAZ:00139401</oboInOwl:id>
        <rdfs:label>Cape Bird</rdfs:label>
    </owl:NamedIndividual>
    


    <!-- http://purl.obolibrary.org/obo/GAZ_00139405 -->

    <owl:NamedIndividual rdf:about="http://purl.obolibrary.org/obo/GAZ_00139405">
        <obo:RO_0001025 rdf:resource="http://purl.obolibrary.org/obo/GAZ_00141552"/>
        <obo:IAO_0000115>An inlet on the SE side of Petermann Island.</obo:IAO_0000115>
        <oboInOwl:hasOBONamespace>GAZ</oboInOwl:hasOBONamespace>
        <oboInOwl:id>GAZ:00139405</oboInOwl:id>
        <rdfs:label>Port Circumcision</rdfs:label>
    </owl:NamedIndividual>
    


    <!-- http://purl.obolibrary.org/obo/GAZ_00139406 -->

    <owl:NamedIndividual rdf:about="http://purl.obolibrary.org/obo/GAZ_00139406">
        <obo:RO_0001025 rdf:resource="http://purl.obolibrary.org/obo/GAZ_00051745"/>
        <obo:IAO_0000115>A glacier-filled fjord separating the Law Peninsula from the Kemp Coast, and opening into Stefannson Bay.</obo:IAO_0000115>
        <oboInOwl:hasOBONamespace>GAZ</oboInOwl:hasOBONamespace>
        <oboInOwl:id>GAZ:00139406</oboInOwl:id>
        <rdfs:label>Cirque Fjord</rdfs:label>
    </owl:NamedIndividual>
    


    <!-- http://purl.obolibrary.org/obo/GAZ_00139412 -->

    <owl:NamedIndividual rdf:about="http://purl.obolibrary.org/obo/GAZ_00139412">
        <obo:RO_0001025 rdf:resource="http://purl.obolibrary.org/obo/GAZ_00051499"/>
        <obo:IAO_0000115>A bay on the Clarie Coast. About 12 miles wide at the entrance between Cape Cesney and Lewis Island.</obo:IAO_0000115>
        <oboInOwl:hasOBONamespace>GAZ</oboInOwl:hasOBONamespace>
        <oboInOwl:id>GAZ:00139412</oboInOwl:id>
        <rdfs:label>Davis Bay</rdfs:label>
    </owl:NamedIndividual>
    


    <!-- http://purl.obolibrary.org/obo/GAZ_00139413 -->

    <owl:NamedIndividual rdf:about="http://purl.obolibrary.org/obo/GAZ_00139413">
        <obo:RO_0001025 rdf:resource="http://purl.obolibrary.org/obo/GAZ_00139412"/>
        <obo:IAO_0000115>A small rocky island rising to 30 m, marking the E side of the entrance to Davis Bay.</obo:IAO_0000115>
        <oboInOwl:hasOBONamespace>GAZ</oboInOwl:hasOBONamespace>
        <oboInOwl:id>GAZ:00139413</oboInOwl:id>
        <rdfs:label>Lewis Island</rdfs:label>
    </owl:NamedIndividual>
    


    <!-- http://purl.obolibrary.org/obo/GAZ_00139414 -->

    <owl:NamedIndividual rdf:about="http://purl.obolibrary.org/obo/GAZ_00139414">
        <obo:RO_0001025 rdf:resource="http://purl.obolibrary.org/obo/GAZ_00140059"/>
        <obo:IAO_0000115>A harbor on the NW side of Robert Island.</obo:IAO_0000115>
        <oboInOwl:hasOBONamespace>GAZ</oboInOwl:hasOBONamespace>
        <oboInOwl:id>GAZ:00139414</oboInOwl:id>
        <rdfs:label>Clothier Harbor</rdfs:label>
    </owl:NamedIndividual>
    


    <!-- http://purl.obolibrary.org/obo/GAZ_00139416 -->

    <owl:NamedIndividual rdf:about="http://purl.obolibrary.org/obo/GAZ_00139416">
        <obo:RO_0001025 rdf:resource="http://purl.obolibrary.org/obo/GAZ_00007425"/>
        <oboInOwl:hasOBONamespace>GAZ</oboInOwl:hasOBONamespace>
        <oboInOwl:id>GAZ:00139416</oboInOwl:id>
        <rdfs:label>Keller Peninsula</rdfs:label>
    </owl:NamedIndividual>
    


    <!-- http://purl.obolibrary.org/obo/GAZ_00139417 -->

    <owl:NamedIndividual rdf:about="http://purl.obolibrary.org/obo/GAZ_00139417">
        <obo:RO_0001025 rdf:resource="http://purl.obolibrary.org/obo/GAZ_00139416"/>
        <obo:IAO_0000115>A Brazilian research station located in Admiralty Bay, King George Island, near the tip of the Antarctic Peninsula. Established 1984.</obo:IAO_0000115>
        <oboInOwl:hasOBONamespace>GAZ</oboInOwl:hasOBONamespace>
        <oboInOwl:id>GAZ:00139417</oboInOwl:id>
        <rdfs:label>Commoandante Ferraz Station</rdfs:label>
    </owl:NamedIndividual>
    


    <!-- http://purl.obolibrary.org/obo/GAZ_00139420 -->

    <owl:NamedIndividual rdf:about="http://purl.obolibrary.org/obo/GAZ_00139420">
        <obo:RO_0001025 rdf:resource="http://purl.obolibrary.org/obo/GAZ_00051499"/>
        <obo:IAO_0000115>An ice shelf on George V Coast, occupying a bay between Cape Freshfield and Cape Hudson.</obo:IAO_0000115>
        <oboInOwl:hasOBONamespace>GAZ</oboInOwl:hasOBONamespace>
        <oboInOwl:id>GAZ:00139420</oboInOwl:id>
        <rdfs:label>Cook Ice Shelf</rdfs:label>
    </owl:NamedIndividual>
    


    <!-- http://purl.obolibrary.org/obo/GAZ_00139422 -->

    <owl:NamedIndividual rdf:about="http://purl.obolibrary.org/obo/GAZ_00139422">
        <obo:RO_0001025 rdf:resource="http://purl.obolibrary.org/obo/GAZ_00000373"/>
        <obo:IAO_0000115>A coastal sea off East Antarctica, between Cape Boothby at 57deg16minE and the W end of the West Ice Shelf, at about 80degE, bordered by the Mawson, Lars Christensen and Ingrid Christensen Coasts. No definitive N boundary.</obo:IAO_0000115>
        <oboInOwl:hasOBONamespace>GAZ</oboInOwl:hasOBONamespace>
        <oboInOwl:id>GAZ:00139422</oboInOwl:id>
        <rdfs:label>Cooperation Sea</rdfs:label>
    </owl:NamedIndividual>
    


    <!-- http://purl.obolibrary.org/obo/GAZ_00139423 -->

    <owl:NamedIndividual rdf:about="http://purl.obolibrary.org/obo/GAZ_00139423">
        <obo:RO_0001025 rdf:resource="http://purl.obolibrary.org/obo/GAZ_00007288"/>
        <obo:IAO_0000115>An ice-free peninsula on the W side of Robert Island.</obo:IAO_0000115>
        <oboInOwl:hasOBONamespace>GAZ</oboInOwl:hasOBONamespace>
        <oboInOwl:id>GAZ:00139423</oboInOwl:id>
        <rdfs:label>Coppermine Peninsula</rdfs:label>
    </owl:NamedIndividual>
    


    <!-- http://purl.obolibrary.org/obo/GAZ_00139424 -->

    <owl:NamedIndividual rdf:about="http://purl.obolibrary.org/obo/GAZ_00139424">
        <obo:RO_0001025 rdf:resource="http://purl.obolibrary.org/obo/GAZ_00014085"/>
        <obo:IAO_0000115>An ice shelf occupying a deep bay between King Peninsula and Canisteo Peninsula.</obo:IAO_0000115>
        <oboInOwl:hasOBONamespace>GAZ</oboInOwl:hasOBONamespace>
        <oboInOwl:id>GAZ:00139424</oboInOwl:id>
        <rdfs:label>Cosgrove Ice Shelf</rdfs:label>
    </owl:NamedIndividual>
    


    <!-- http://purl.obolibrary.org/obo/GAZ_00139428 -->

    <owl:NamedIndividual rdf:about="http://purl.obolibrary.org/obo/GAZ_00139428">
        <obo:RO_0001025 rdf:resource="http://purl.obolibrary.org/obo/GAZ_00014085"/>
        <obo:IAO_0000115>An ice shelf in a bay formed by an arm of the Bear Peninsula.</obo:IAO_0000115>
        <oboInOwl:hasOBONamespace>GAZ</oboInOwl:hasOBONamespace>
        <oboInOwl:id>GAZ:00139428</oboInOwl:id>
        <rdfs:label>Crosson Ice Shelf</rdfs:label>
    </owl:NamedIndividual>
    


    <!-- http://purl.obolibrary.org/obo/GAZ_00139429 -->

    <owl:NamedIndividual rdf:about="http://purl.obolibrary.org/obo/GAZ_00139429">
        <obo:RO_0001025 rdf:resource="http://purl.obolibrary.org/obo/GAZ_00141552"/>
        <obo:IAO_0000115>A broad waterway between the Briscoe Islands and Graham Land, extending S to Liard Island.</obo:IAO_0000115>
        <oboInOwl:hasOBONamespace>GAZ</oboInOwl:hasOBONamespace>
        <oboInOwl:id>GAZ:00139429</oboInOwl:id>
        <rdfs:label>Crystal Sound</rdfs:label>
    </owl:NamedIndividual>
    


    <!-- http://purl.obolibrary.org/obo/GAZ_00139431 -->

    <owl:NamedIndividual rdf:about="http://purl.obolibrary.org/obo/GAZ_00139431">
        <obo:RO_0001025 rdf:resource="http://purl.obolibrary.org/obo/GAZ_00007425"/>
        <obo:IAO_0000115>A German research station in Potter Cove.</obo:IAO_0000115>
        <oboInOwl:hasOBONamespace>GAZ</oboInOwl:hasOBONamespace>
        <oboInOwl:id>GAZ:00139431</oboInOwl:id>
        <rdfs:label>Dallman Laboratory</rdfs:label>
    </owl:NamedIndividual>
    


    <!-- http://purl.obolibrary.org/obo/GAZ_00139432 -->

    <owl:NamedIndividual rdf:about="http://purl.obolibrary.org/obo/GAZ_00139432">
        <obo:RO_0001025 rdf:resource="http://purl.obolibrary.org/obo/GAZ_00140059"/>
        <obo:IAO_0000115>A cove indenting the SW side of King George Island to the E of Barton Peninsula, in the South Shetland Islands.</obo:IAO_0000115>
        <oboInOwl:hasOBONamespace>GAZ</oboInOwl:hasOBONamespace>
        <oboInOwl:id>GAZ:00139432</oboInOwl:id>
        <rdfs:label>Potter Cove</rdfs:label>
    </owl:NamedIndividual>
    


    <!-- http://purl.obolibrary.org/obo/GAZ_00139433 -->

    <owl:NamedIndividual rdf:about="http://purl.obolibrary.org/obo/GAZ_00139433">
        <rdf:type rdf:resource="http://purl.obolibrary.org/obo/ENVO_00000305"/>
        <obo:RO_0001025 rdf:resource="http://purl.obolibrary.org/obo/GAZ_00045055"/>
        <obo:IAO_0000115>A headland on Wiencke Island.</obo:IAO_0000115>
        <oboInOwl:hasOBONamespace>GAZ</oboInOwl:hasOBONamespace>
        <oboInOwl:id>GAZ:00139433</oboInOwl:id>
        <rdfs:label>Damoy Point</rdfs:label>
    </owl:NamedIndividual>
    


    <!-- http://purl.obolibrary.org/obo/GAZ_00139434 -->

    <owl:NamedIndividual rdf:about="http://purl.obolibrary.org/obo/GAZ_00139434">
        <obo:RO_0001025 rdf:resource="http://purl.obolibrary.org/obo/GAZ_00045049"/>
        <obo:IAO_0000115>A former (1956-1959) British research station.</obo:IAO_0000115>
        <oboInOwl:hasOBONamespace>GAZ</oboInOwl:hasOBONamespace>
        <oboInOwl:id>GAZ:00139434</oboInOwl:id>
        <rdfs:label>Base O</rdfs:label>
    </owl:NamedIndividual>
    


    <!-- http://purl.obolibrary.org/obo/GAZ_00139437 -->

    <owl:NamedIndividual rdf:about="http://purl.obolibrary.org/obo/GAZ_00139437">
        <obo:RO_0001025 rdf:resource="http://purl.obolibrary.org/obo/GAZ_00014121"/>
        <obo:IAO_0000115>An Argentine research station in Fumerole Cove.</obo:IAO_0000115>
        <oboInOwl:hasOBONamespace>GAZ</oboInOwl:hasOBONamespace>
        <oboInOwl:id>GAZ:00139437</oboInOwl:id>
        <rdfs:label>Decepcion Station</rdfs:label>
    </owl:NamedIndividual>
    


    <!-- http://purl.obolibrary.org/obo/GAZ_00139438 -->

    <owl:NamedIndividual rdf:about="http://purl.obolibrary.org/obo/GAZ_00139438">
        <obo:RO_0001025 rdf:resource="http://purl.obolibrary.org/obo/GAZ_00014121"/>
        <obo:IAO_0000115>A former (1943-1959) British research station at Whalers Bay.</obo:IAO_0000115>
        <oboInOwl:hasOBONamespace>GAZ</oboInOwl:hasOBONamespace>
        <oboInOwl:id>GAZ:00139438</oboInOwl:id>
        <rdfs:label>Base B</rdfs:label>
    </owl:NamedIndividual>
    


    <!-- http://purl.obolibrary.org/obo/GAZ_00139440 -->

    <owl:NamedIndividual rdf:about="http://purl.obolibrary.org/obo/GAZ_00139440">
        <obo:RO_0001025 rdf:resource="http://purl.obolibrary.org/obo/GAZ_00139496"/>
        <obo:IAO_0000115>A small bay entered between Fildes Point and Penfold Point at the E side of Port Foster, Deception Island, in the South Shetland Islands.</obo:IAO_0000115>
        <oboInOwl:hasOBONamespace>GAZ</oboInOwl:hasOBONamespace>
        <oboInOwl:id>GAZ:00139440</oboInOwl:id>
        <rdfs:label>Whalers Bay</rdfs:label>
    </owl:NamedIndividual>
    


    <!-- http://purl.obolibrary.org/obo/GAZ_00139441 -->

    <owl:NamedIndividual rdf:about="http://purl.obolibrary.org/obo/GAZ_00139441">
        <obo:RO_0001025 rdf:resource="http://purl.obolibrary.org/obo/GAZ_00014121"/>
        <obo:IAO_0000115>A Spanish research station. Established 1989.</obo:IAO_0000115>
        <oboInOwl:hasOBONamespace>GAZ</oboInOwl:hasOBONamespace>
        <oboInOwl:id>GAZ:00139441</oboInOwl:id>
        <rdfs:label>Gabriele de Castilla Station</rdfs:label>
    </owl:NamedIndividual>
    


    <!-- http://purl.obolibrary.org/obo/GAZ_00139442 -->

    <owl:NamedIndividual rdf:about="http://purl.obolibrary.org/obo/GAZ_00139442">
        <obo:RO_0001025 rdf:resource="http://purl.obolibrary.org/obo/GAZ_00139496"/>
        <oboInOwl:hasOBONamespace>GAZ</oboInOwl:hasOBONamespace>
        <oboInOwl:id>GAZ:00139442</oboInOwl:id>
        <rdfs:label>Pendulum Cove</rdfs:label>
    </owl:NamedIndividual>
    


    <!-- http://purl.obolibrary.org/obo/GAZ_00139443 -->

    <owl:NamedIndividual rdf:about="http://purl.obolibrary.org/obo/GAZ_00139443">
        <obo:RO_0001025 rdf:resource="http://purl.obolibrary.org/obo/GAZ_00014121"/>
        <obo:IAO_0000115>A former Chilean research station on Pendulum Cove. Destoyed by fire.</obo:IAO_0000115>
        <oboInOwl:hasOBONamespace>GAZ</oboInOwl:hasOBONamespace>
        <oboInOwl:id>GAZ:00139443</oboInOwl:id>
        <rdfs:label>Presidente Pedro Aguirre Cerda Station</rdfs:label>
    </owl:NamedIndividual>
    


    <!-- http://purl.obolibrary.org/obo/GAZ_00139444 -->

    <owl:NamedIndividual rdf:about="http://purl.obolibrary.org/obo/GAZ_00139444">
        <obo:RO_0001025 rdf:resource="http://purl.obolibrary.org/obo/GAZ_00007328"/>
        <obo:IAO_0000115>Rocks off Baily Head, Deception Island.</obo:IAO_0000115>
        <oboInOwl:hasOBONamespace>GAZ</oboInOwl:hasOBONamespace>
        <oboInOwl:id>GAZ:00139444</oboInOwl:id>
        <rdfs:label>Sewing Machine Needles</rdfs:label>
    </owl:NamedIndividual>
    


    <!-- http://purl.obolibrary.org/obo/GAZ_00139445 -->

    <owl:NamedIndividual rdf:about="http://purl.obolibrary.org/obo/GAZ_00139445">
        <obo:RO_0001025 rdf:resource="http://purl.obolibrary.org/obo/GAZ_00139496"/>
        <obo:IAO_0000115>A small bay in the northwest side of Port Foster, Deception Island, in the South Shetland Islands.</obo:IAO_0000115>
        <oboInOwl:hasOBONamespace>GAZ</oboInOwl:hasOBONamespace>
        <oboInOwl:id>GAZ:00139445</oboInOwl:id>
        <rdfs:label>Telefon Bay</rdfs:label>
    </owl:NamedIndividual>
    


    <!-- http://purl.obolibrary.org/obo/GAZ_00139446 -->

    <owl:NamedIndividual rdf:about="http://purl.obolibrary.org/obo/GAZ_00139446">
        <obo:RO_0001025 rdf:resource="http://purl.obolibrary.org/obo/GAZ_00014121"/>
        <obo:RO_0001025 rdf:resource="http://purl.obolibrary.org/obo/GAZ_00140059"/>
        <obo:IAO_0000115>The narrow entrance into the inner flooded crater of Deception Island.</obo:IAO_0000115>
        <oboInOwl:hasOBONamespace>GAZ</oboInOwl:hasOBONamespace>
        <oboInOwl:id>GAZ:00139446</oboInOwl:id>
        <rdfs:label>Neptunes Bellows</rdfs:label>
    </owl:NamedIndividual>
    


    <!-- http://purl.obolibrary.org/obo/GAZ_00139447 -->

    <owl:NamedIndividual rdf:about="http://purl.obolibrary.org/obo/GAZ_00139447">
        <obo:RO_0001025 rdf:resource="http://purl.obolibrary.org/obo/GAZ_00014121"/>
        <obo:IAO_0000115>The NE point of Deception Island.</obo:IAO_0000115>
        <oboInOwl:hasOBONamespace>GAZ</oboInOwl:hasOBONamespace>
        <oboInOwl:id>GAZ:00139447</oboInOwl:id>
        <rdfs:label>Macaroni Point</rdfs:label>
    </owl:NamedIndividual>
    


    <!-- http://purl.obolibrary.org/obo/GAZ_00139448 -->

    <owl:NamedIndividual rdf:about="http://purl.obolibrary.org/obo/GAZ_00139448">
        <obo:RO_0001025 rdf:resource="http://purl.obolibrary.org/obo/GAZ_00139449"/>
        <obo:IAO_0000115>An island in Lallemand Fjord.</obo:IAO_0000115>
        <oboInOwl:hasOBONamespace>GAZ</oboInOwl:hasOBONamespace>
        <oboInOwl:id>GAZ:00139448</oboInOwl:id>
        <rdfs:label>Detaille Island</rdfs:label>
    </owl:NamedIndividual>
    


    <!-- http://purl.obolibrary.org/obo/GAZ_00139449 -->

    <owl:NamedIndividual rdf:about="http://purl.obolibrary.org/obo/GAZ_00139449">
        <obo:RO_0001025 rdf:resource="http://purl.obolibrary.org/obo/GAZ_00141552"/>
        <obo:IAO_0000115>A fjord on the Loubet Coast, Graham Land.</obo:IAO_0000115>
        <oboInOwl:hasOBONamespace>GAZ</oboInOwl:hasOBONamespace>
        <oboInOwl:id>GAZ:00139449</oboInOwl:id>
        <rdfs:label>Lallemand Fjord</rdfs:label>
    </owl:NamedIndividual>
    


    <!-- http://purl.obolibrary.org/obo/GAZ_00139450 -->

    <owl:NamedIndividual rdf:about="http://purl.obolibrary.org/obo/GAZ_00139450">
        <obo:RO_0001025 rdf:resource="http://purl.obolibrary.org/obo/GAZ_00139448"/>
        <obo:IAO_0000115>A former (1956-1959) British research station.</obo:IAO_0000115>
        <oboInOwl:hasOBONamespace>GAZ</oboInOwl:hasOBONamespace>
        <oboInOwl:id>GAZ:00139450</oboInOwl:id>
        <rdfs:label>Base W</rdfs:label>
    </owl:NamedIndividual>
    


    <!-- http://purl.obolibrary.org/obo/GAZ_00139452 -->

    <owl:NamedIndividual rdf:about="http://purl.obolibrary.org/obo/GAZ_00139452">
        <obo:RO_0001025 rdf:resource="http://purl.obolibrary.org/obo/GAZ_00014089"/>
        <obo:IAO_0000115>A group of islands 14 km S of Adelaide Island.</obo:IAO_0000115>
        <oboInOwl:hasOBONamespace>GAZ</oboInOwl:hasOBONamespace>
        <oboInOwl:id>GAZ:00139452</oboInOwl:id>
        <rdfs:label>Dion Islands</rdfs:label>
    </owl:NamedIndividual>
    


    <!-- http://purl.obolibrary.org/obo/GAZ_00139453 -->

    <owl:NamedIndividual rdf:about="http://purl.obolibrary.org/obo/GAZ_00139453">
        <obo:RO_0001025 rdf:resource="http://purl.obolibrary.org/obo/GAZ_00140059"/>
        <obo:IAO_0000115>A bay on the N coast of Greenwich Island.</obo:IAO_0000115>
        <oboInOwl:hasOBONamespace>GAZ</oboInOwl:hasOBONamespace>
        <oboInOwl:id>GAZ:00139453</oboInOwl:id>
        <rdfs:label>Discovery Bay</rdfs:label>
    </owl:NamedIndividual>
    


    <!-- http://purl.obolibrary.org/obo/GAZ_00139454 -->

    <owl:NamedIndividual rdf:about="http://purl.obolibrary.org/obo/GAZ_00139454">
        <obo:RO_0001025 rdf:resource="http://purl.obolibrary.org/obo/GAZ_00141552"/>
        <obo:IAO_0000115>A narrow channel off Briggs Peninsula, Anvers Island.</obo:IAO_0000115>
        <oboInOwl:hasOBONamespace>GAZ</oboInOwl:hasOBONamespace>
        <oboInOwl:id>GAZ:00139454</oboInOwl:id>
        <rdfs:label>Discovery Channel</rdfs:label>
    </owl:NamedIndividual>
    


    <!-- http://purl.obolibrary.org/obo/GAZ_00139457 -->

    <owl:NamedIndividual rdf:about="http://purl.obolibrary.org/obo/GAZ_00139457">
        <obo:RO_0001025 rdf:resource="http://purl.obolibrary.org/obo/GAZ_00014085"/>
        <obo:IAO_0000115>An ice shelf between the Bear Peninsula and Martin Peninsula.</obo:IAO_0000115>
        <oboInOwl:hasOBONamespace>GAZ</oboInOwl:hasOBONamespace>
        <oboInOwl:id>GAZ:00139457</oboInOwl:id>
        <rdfs:label>Dotson Ice Shelf</rdfs:label>
    </owl:NamedIndividual>
    


    <!-- http://purl.obolibrary.org/obo/GAZ_00139459 -->

    <owl:NamedIndividual rdf:about="http://purl.obolibrary.org/obo/GAZ_00139459">
        <obo:RO_0001025 rdf:resource="http://purl.obolibrary.org/obo/GAZ_00139739"/>
        <obo:IAO_0000115>An ice shelf bordering the Weddell Sea, between Berkner Island and the Luitpold Coast.</obo:IAO_0000115>
        <oboInOwl:hasOBONamespace>GAZ</oboInOwl:hasOBONamespace>
        <oboInOwl:id>GAZ:00139459</oboInOwl:id>
        <rdfs:label>Filchner Ice Shelf</rdfs:label>
    </owl:NamedIndividual>
    


    <!-- http://purl.obolibrary.org/obo/GAZ_00139460 -->

    <owl:NamedIndividual rdf:about="http://purl.obolibrary.org/obo/GAZ_00139460">
        <obo:RO_0001025 rdf:resource="http://purl.obolibrary.org/obo/GAZ_00139459"/>
        <obo:IAO_0000115>A United States research station.</obo:IAO_0000115>
        <oboInOwl:hasOBONamespace>GAZ</oboInOwl:hasOBONamespace>
        <oboInOwl:id>GAZ:00139460</oboInOwl:id>
        <rdfs:label>Ellsworth Station</rdfs:label>
    </owl:NamedIndividual>
    


    <!-- http://purl.obolibrary.org/obo/GAZ_00139461 -->

    <owl:NamedIndividual rdf:about="http://purl.obolibrary.org/obo/GAZ_00139461">
        <obo:RO_0001025 rdf:resource="http://purl.obolibrary.org/obo/GAZ_00139459"/>
        <obo:IAO_0000115>A former (1976-1986/1987) Russian research station.</obo:IAO_0000115>
        <oboInOwl:hasOBONamespace>GAZ</oboInOwl:hasOBONamespace>
        <oboInOwl:id>GAZ:00139461</oboInOwl:id>
        <rdfs:label>Druzhnaya I</rdfs:label>
    </owl:NamedIndividual>
    


    <!-- http://purl.obolibrary.org/obo/GAZ_00139462 -->

    <owl:NamedIndividual rdf:about="http://purl.obolibrary.org/obo/GAZ_00139462">
        <obo:RO_0001025 rdf:resource="http://purl.obolibrary.org/obo/GAZ_00139459"/>
        <obo:IAO_0000115>An Argentine research station.</obo:IAO_0000115>
        <oboInOwl:hasOBONamespace>GAZ</oboInOwl:hasOBONamespace>
        <oboInOwl:id>GAZ:00139462</oboInOwl:id>
        <rdfs:label>General Belgrano Station</rdfs:label>
    </owl:NamedIndividual>
    


    <!-- http://purl.obolibrary.org/obo/GAZ_00139463 -->

    <owl:NamedIndividual rdf:about="http://purl.obolibrary.org/obo/GAZ_00139463">
        <obo:RO_0001025 rdf:resource="http://purl.obolibrary.org/obo/GAZ_00139739"/>
        <obo:IAO_0000115>A large ice shelf bordering the Weddell Sea extending from the E coast of Palmer Land and Berkener Island S to Ellsworth Land.</obo:IAO_0000115>
        <oboInOwl:hasOBONamespace>GAZ</oboInOwl:hasOBONamespace>
        <oboInOwl:id>GAZ:00139463</oboInOwl:id>
        <rdfs:label>Ronne Ice Shelf</rdfs:label>
    </owl:NamedIndividual>
    


    <!-- http://purl.obolibrary.org/obo/GAZ_00139464 -->

    <owl:NamedIndividual rdf:about="http://purl.obolibrary.org/obo/GAZ_00139464">
        <obo:RO_0001025 rdf:resource="http://purl.obolibrary.org/obo/GAZ_00139463"/>
        <obo:IAO_0000115>A Russian research station, established 1980.</obo:IAO_0000115>
        <oboInOwl:hasOBONamespace>GAZ</oboInOwl:hasOBONamespace>
        <oboInOwl:id>GAZ:00139464</oboInOwl:id>
        <rdfs:label>Druzhnaya II</rdfs:label>
    </owl:NamedIndividual>
    


    <!-- http://purl.obolibrary.org/obo/GAZ_00139466 -->

    <owl:NamedIndividual rdf:about="http://purl.obolibrary.org/obo/GAZ_00139466">
        <obo:RO_0001025 rdf:resource="http://purl.obolibrary.org/obo/GAZ_00003703"/>
        <obo:IAO_0000115>A Russian research station. Established 1987.</obo:IAO_0000115>
        <oboInOwl:hasOBONamespace>GAZ</oboInOwl:hasOBONamespace>
        <oboInOwl:id>GAZ:00139466</oboInOwl:id>
        <rdfs:label>Druzhnaya IV</rdfs:label>
    </owl:NamedIndividual>
    


    <!-- http://purl.obolibrary.org/obo/GAZ_00139474 -->

    <owl:NamedIndividual rdf:about="http://purl.obolibrary.org/obo/GAZ_00139474">
        <obo:RO_0001025 rdf:resource="http://purl.obolibrary.org/obo/GAZ_00014090"/>
        <obo:IAO_0000115>A group of islands which rise through the ice near the SW end of George VI Sound.</obo:IAO_0000115>
        <oboInOwl:hasOBONamespace>GAZ</oboInOwl:hasOBONamespace>
        <oboInOwl:id>GAZ:00139474</oboInOwl:id>
        <rdfs:label>Eklund Islands</rdfs:label>
    </owl:NamedIndividual>
    


    <!-- http://purl.obolibrary.org/obo/GAZ_00139475 -->

    <owl:NamedIndividual rdf:about="http://purl.obolibrary.org/obo/GAZ_00139475">
        <obo:RO_0001025 rdf:resource="http://purl.obolibrary.org/obo/GAZ_00141024"/>
        <obo:IAO_0000115>A harbor between Christoffersen Island and Michelsen Island.</obo:IAO_0000115>
        <oboInOwl:hasOBONamespace>GAZ</oboInOwl:hasOBONamespace>
        <oboInOwl:id>GAZ:00139475</oboInOwl:id>
        <rdfs:label>Ellefsen Harbour</rdfs:label>
    </owl:NamedIndividual>
    


    <!-- http://purl.obolibrary.org/obo/GAZ_00139476 -->

    <owl:NamedIndividual rdf:about="http://purl.obolibrary.org/obo/GAZ_00139476">
        <obo:RO_0001025 rdf:resource="http://purl.obolibrary.org/obo/GAZ_00139452"/>
        <obo:IAO_0000115>One of the Dion Islands, at the N entrance to Marguerite Bay.</obo:IAO_0000115>
        <oboInOwl:hasOBONamespace>GAZ</oboInOwl:hasOBONamespace>
        <oboInOwl:id>GAZ:00139476</oboInOwl:id>
        <rdfs:label>Emperor Island</rdfs:label>
    </owl:NamedIndividual>
    


    <!-- http://purl.obolibrary.org/obo/GAZ_00139477 -->

    <owl:NamedIndividual rdf:about="http://purl.obolibrary.org/obo/GAZ_00139477">
        <obo:RO_0001025 rdf:resource="http://purl.obolibrary.org/obo/GAZ_00007425"/>
        <obo:IAO_0000115>A Chilean research station.</obo:IAO_0000115>
        <oboInOwl:hasOBONamespace>GAZ</oboInOwl:hasOBONamespace>
        <oboInOwl:id>GAZ:00139477</oboInOwl:id>
        <rdfs:label>Professor Julio Escudero Base</rdfs:label>
    </owl:NamedIndividual>
    


    <!-- http://purl.obolibrary.org/obo/GAZ_00139480 -->

    <owl:NamedIndividual rdf:about="http://purl.obolibrary.org/obo/GAZ_00139480">
        <obo:RO_0001025 rdf:resource="http://purl.obolibrary.org/obo/GAZ_00139481"/>
        <obo:IAO_0000115>A harbor in Venus Bay.</obo:IAO_0000115>
        <oboInOwl:hasOBONamespace>GAZ</oboInOwl:hasOBONamespace>
        <oboInOwl:id>GAZ:00139480</oboInOwl:id>
        <rdfs:label>Esther Harbour</rdfs:label>
    </owl:NamedIndividual>
    


    <!-- http://purl.obolibrary.org/obo/GAZ_00139481 -->

    <owl:NamedIndividual rdf:about="http://purl.obolibrary.org/obo/GAZ_00139481">
        <obo:RO_0001025 rdf:resource="http://purl.obolibrary.org/obo/GAZ_00140059"/>
        <obo:IAO_0000115>A bay on the N coast of King George Island.</obo:IAO_0000115>
        <oboInOwl:hasOBONamespace>GAZ</oboInOwl:hasOBONamespace>
        <oboInOwl:id>GAZ:00139481</oboInOwl:id>
        <rdfs:label>Venus Bay</rdfs:label>
    </owl:NamedIndividual>
    


    <!-- http://purl.obolibrary.org/obo/GAZ_00139482 -->

    <owl:NamedIndividual rdf:about="http://purl.obolibrary.org/obo/GAZ_00139482">
        <obo:RO_0001025 rdf:resource="http://purl.obolibrary.org/obo/GAZ_00014089"/>
        <obo:IAO_0000115>An ice shelf in Marguerite Bay, on the Fallieres Coast. It occupies the inlet between Cape Breteaux and Mount Edgell. Now almost disappeared.</obo:IAO_0000115>
        <oboInOwl:hasOBONamespace>GAZ</oboInOwl:hasOBONamespace>
        <oboInOwl:id>GAZ:00139482</oboInOwl:id>
        <rdfs:label>Wordie Ice Shelf</rdfs:label>
    </owl:NamedIndividual>
    


    <!-- http://purl.obolibrary.org/obo/GAZ_00139484 -->

    <owl:NamedIndividual rdf:about="http://purl.obolibrary.org/obo/GAZ_00139484">
        <obo:RO_0001025 rdf:resource="http://purl.obolibrary.org/obo/GAZ_00014089"/>
        <obo:IAO_0000115>A group of small rocky islands in central Marguerite Bay.</obo:IAO_0000115>
        <oboInOwl:hasOBONamespace>GAZ</oboInOwl:hasOBONamespace>
        <oboInOwl:id>GAZ:00139484</oboInOwl:id>
        <rdfs:label>Faure Islands</rdfs:label>
    </owl:NamedIndividual>
    


    <!-- http://purl.obolibrary.org/obo/GAZ_00139487 -->

    <owl:NamedIndividual rdf:about="http://purl.obolibrary.org/obo/GAZ_00139487">
        <obo:RO_0001025 rdf:resource="http://purl.obolibrary.org/obo/GAZ_00140059"/>
        <obo:IAO_0000115>The strait between King George Island and Nelson Island.</obo:IAO_0000115>
        <oboInOwl:hasOBONamespace>GAZ</oboInOwl:hasOBONamespace>
        <oboInOwl:id>GAZ:00139487</oboInOwl:id>
        <rdfs:label>Fildes Strait</rdfs:label>
    </owl:NamedIndividual>
    


    <!-- http://purl.obolibrary.org/obo/GAZ_00139488 -->

    <owl:NamedIndividual rdf:about="http://purl.obolibrary.org/obo/GAZ_00139488">
        <obo:RO_0001025 rdf:resource="http://purl.obolibrary.org/obo/GAZ_00141554"/>
        <obo:IAO_0000115>An ice shelf bordering Kronprincesse Martha Kyst.</obo:IAO_0000115>
        <oboInOwl:hasOBONamespace>GAZ</oboInOwl:hasOBONamespace>
        <oboInOwl:id>GAZ:00139488</oboInOwl:id>
        <rdfs:label>Fimbulisen</rdfs:label>
    </owl:NamedIndividual>
    


    <!-- http://purl.obolibrary.org/obo/GAZ_00139493 -->

    <owl:NamedIndividual rdf:about="http://purl.obolibrary.org/obo/GAZ_00139493">
        <obo:RO_0001025 rdf:resource="http://purl.obolibrary.org/obo/GAZ_00014088"/>
        <oboInOwl:hasOBONamespace>GAZ</oboInOwl:hasOBONamespace>
        <oboInOwl:id>GAZ:00139493</oboInOwl:id>
        <rdfs:label>Fossil Bluff</rdfs:label>
    </owl:NamedIndividual>
    


    <!-- http://purl.obolibrary.org/obo/GAZ_00139494 -->

    <owl:NamedIndividual rdf:about="http://purl.obolibrary.org/obo/GAZ_00139494">
        <obo:RO_0001025 rdf:resource="http://purl.obolibrary.org/obo/GAZ_00139493"/>
        <obo:IAO_0000115>A British research station, built 1961-02.</obo:IAO_0000115>
        <oboInOwl:hasOBONamespace>GAZ</oboInOwl:hasOBONamespace>
        <oboInOwl:id>GAZ:00139494</oboInOwl:id>
        <rdfs:label>Fossil Bluff Station</rdfs:label>
    </owl:NamedIndividual>
    


    <!-- http://purl.obolibrary.org/obo/GAZ_00139496 -->

    <owl:NamedIndividual rdf:about="http://purl.obolibrary.org/obo/GAZ_00139496">
        <obo:RO_0001025 rdf:resource="http://purl.obolibrary.org/obo/GAZ_00140059"/>
        <obo:IAO_0000115>The inner harbor of Deception Island.</obo:IAO_0000115>
        <oboInOwl:hasOBONamespace>GAZ</oboInOwl:hasOBONamespace>
        <oboInOwl:id>GAZ:00139496</oboInOwl:id>
        <rdfs:label>Port Forster</rdfs:label>
    </owl:NamedIndividual>
    


    <!-- http://purl.obolibrary.org/obo/GAZ_00139497 -->

    <owl:NamedIndividual rdf:about="http://purl.obolibrary.org/obo/GAZ_00139497">
        <obo:RO_0001025 rdf:resource="http://purl.obolibrary.org/obo/GAZ_00045019"/>
        <obo:IAO_0000115>A harbor between Nansen Island and Enterprise Island.</obo:IAO_0000115>
        <oboInOwl:hasOBONamespace>GAZ</oboInOwl:hasOBONamespace>
        <oboInOwl:id>GAZ:00139497</oboInOwl:id>
        <rdfs:label>Foyn Harbour</rdfs:label>
    </owl:NamedIndividual>
    


    <!-- http://purl.obolibrary.org/obo/GAZ_00139595 -->

    <owl:NamedIndividual rdf:about="http://purl.obolibrary.org/obo/GAZ_00139595">
        <obo:RO_0001025 rdf:resource="http://purl.obolibrary.org/obo/GAZ_00139150"/>
        <obo:IAO_0000115>An island nearly 5 mi long, lying 3 mi SW of D&apos;Urville Island off the NE end of Antarctic Peninsula.</obo:IAO_0000115>
        <oboInOwl:hasOBONamespace>GAZ</oboInOwl:hasOBONamespace>
        <oboInOwl:id>GAZ:00139595</oboInOwl:id>
        <rdfs:label>Bransfield Island</rdfs:label>
    </owl:NamedIndividual>
    


    <!-- http://purl.obolibrary.org/obo/GAZ_00139596 -->

    <owl:NamedIndividual rdf:about="http://purl.obolibrary.org/obo/GAZ_00139596">
        <obo:RO_0001025 rdf:resource="http://purl.obolibrary.org/obo/GAZ_00051499"/>
        <obo:IAO_0000115>A sheltered bay about 1.6 km in extent, between Clark Peninsula and Bailey Peninsula in the Windmill Islands.</obo:IAO_0000115>
        <oboInOwl:hasOBONamespace>GAZ</oboInOwl:hasOBONamespace>
        <oboInOwl:id>GAZ:00139596</oboInOwl:id>
        <rdfs:label>Newcomb Bay</rdfs:label>
    </owl:NamedIndividual>
    


    <!-- http://purl.obolibrary.org/obo/GAZ_00139739 -->

    <owl:NamedIndividual rdf:about="http://purl.obolibrary.org/obo/GAZ_00139739">
        <obo:RO_0001025 rdf:resource="http://purl.obolibrary.org/obo/GAZ_00004045"/>
        <obo:IAO_0000115>An ice shelf in Antarctica bordering the Weddell Sea. The seaward side of the Filchner-Ronne ice shelf is divided into Eastern (Filchner) and the larger Western (Ronne) sections by Berkner Island.</obo:IAO_0000115>
        <oboInOwl:hasOBONamespace>GAZ</oboInOwl:hasOBONamespace>
        <oboInOwl:id>GAZ:00139739</oboInOwl:id>
        <rdfs:label>Filchner-Ronne Ice Shelf</rdfs:label>
    </owl:NamedIndividual>
    


    <!-- http://purl.obolibrary.org/obo/GAZ_00139741 -->

    <owl:NamedIndividual rdf:about="http://purl.obolibrary.org/obo/GAZ_00139741">
        <obo:RO_0001025 rdf:resource="http://purl.obolibrary.org/obo/GAZ_00139422"/>
        <obo:IAO_0000115>An open bay in the Antarctic coastal angle formed by the coast and the western end of the West Ice Shelf.</obo:IAO_0000115>
        <oboInOwl:hasOBONamespace>GAZ</oboInOwl:hasOBONamespace>
        <oboInOwl:id>GAZ:00139741</oboInOwl:id>
        <rdfs:label>Barrier Bay</rdfs:label>
    </owl:NamedIndividual>
    


    <!-- http://purl.obolibrary.org/obo/GAZ_00139746 -->

    <owl:NamedIndividual rdf:about="http://purl.obolibrary.org/obo/GAZ_00139746">
        <obo:RO_0001025 rdf:resource="http://purl.obolibrary.org/obo/GAZ_00007329"/>
        <obo:IAO_0000115>A glacier on Livingston Island, Antarctica. It is bounded by the southeastern slopes of Oryahovo Heights and the northwestern slopes of Snow Peak. It extends 5km in east-west direction and 3km in the north-south direction, and drains northeastwards into Hero Bay between Avitohol Point and Remetalk Point.</obo:IAO_0000115>
        <oboInOwl:hasOBONamespace>GAZ</oboInOwl:hasOBONamespace>
        <oboInOwl:id>GAZ:00139746</oboInOwl:id>
        <rdfs:label>Berkovitsa Glacier</rdfs:label>
    </owl:NamedIndividual>
    


    <!-- http://purl.obolibrary.org/obo/GAZ_00139747 -->

    <owl:NamedIndividual rdf:about="http://purl.obolibrary.org/obo/GAZ_00139747">
        <rdf:type rdf:resource="http://purl.obolibrary.org/obo/ENVO_00000305"/>
        <obo:RO_0001025 rdf:resource="http://purl.obolibrary.org/obo/GAZ_00007329"/>
        <obo:IAO_0000115>A headland on the east coast of the Ioannes Paulus II Peninsula, Livingston Island, Antarctica formed by an offshoot of Oryahovo Heights.</obo:IAO_0000115>
        <oboInOwl:hasOBONamespace>GAZ</oboInOwl:hasOBONamespace>
        <oboInOwl:id>GAZ:00139747</oboInOwl:id>
        <rdfs:label>Remetalk Point</rdfs:label>
    </owl:NamedIndividual>
    


    <!-- http://purl.obolibrary.org/obo/GAZ_00139748 -->

    <owl:NamedIndividual rdf:about="http://purl.obolibrary.org/obo/GAZ_00139748">
        <rdf:type rdf:resource="http://purl.obolibrary.org/obo/ENVO_00000305"/>
        <obo:RO_0001025 rdf:resource="http://purl.obolibrary.org/obo/GAZ_00007329"/>
        <obo:IAO_0000115>A headland on the north coast of Livingston Island, Antarctica projecting 700 m into Hero Bay.</obo:IAO_0000115>
        <oboInOwl:hasOBONamespace>GAZ</oboInOwl:hasOBONamespace>
        <oboInOwl:id>GAZ:00139748</oboInOwl:id>
        <rdfs:label>Avitohol Point</rdfs:label>
    </owl:NamedIndividual>
    


    <!-- http://purl.obolibrary.org/obo/GAZ_00139750 -->

    <owl:NamedIndividual rdf:about="http://purl.obolibrary.org/obo/GAZ_00139750">
        <obo:RO_0001025 rdf:resource="http://purl.obolibrary.org/obo/GAZ_00007329"/>
        <obo:IAO_0000115>An ice-covered peninsula on the north coast of Livingston Island, Antarctica that is bounded by Hero Bay to the east and Barclay Bay to the west. It extends 12.8 km in length and is 8.5 km wide. Its northern extremity is formed by the ice-free Cape Shirreff.</obo:IAO_0000115>
        <oboInOwl:hasOBONamespace>GAZ</oboInOwl:hasOBONamespace>
        <oboInOwl:id>GAZ:00139750</oboInOwl:id>
        <rdfs:label>Ioannes Paulus II Peninsula</rdfs:label>
    </owl:NamedIndividual>
    


    <!-- http://purl.obolibrary.org/obo/GAZ_00139751 -->

    <owl:NamedIndividual rdf:about="http://purl.obolibrary.org/obo/GAZ_00139751">
        <obo:RO_0001025 rdf:resource="http://purl.obolibrary.org/obo/GAZ_00139750"/>
        <obo:IAO_0000115>A prominent cape at the north end of the rocky Ioannes Paulus II Peninsula which separates Hero and Barclay Bay on the north coast of Livingston Island, in the South Shetland Islands.</obo:IAO_0000115>
        <oboInOwl:hasOBONamespace>GAZ</oboInOwl:hasOBONamespace>
        <oboInOwl:id>GAZ:00139751</oboInOwl:id>
        <rdfs:label>Cape Shirreff</rdfs:label>
    </owl:NamedIndividual>
    


    <!-- http://purl.obolibrary.org/obo/GAZ_00139752 -->

    <owl:NamedIndividual rdf:about="http://purl.obolibrary.org/obo/GAZ_00139752">
        <obo:RO_0001025 rdf:resource="http://purl.obolibrary.org/obo/GAZ_00140059"/>
        <obo:IAO_0000115>A 17 mi wide bay, which indents for 6 mi the north side of Livingston Island between Cape Shirreff and Williams Point, in the South Shetland Islands. The name Blythe Bay, originally applied to a small bay on the southeast side of Desolation Island on Powell&apos;s chart of 1822 published by Laurie, was erroneously transferred to this bay in the l930s.</obo:IAO_0000115>
        <oboInOwl:hasOBONamespace>GAZ</oboInOwl:hasOBONamespace>
        <oboInOwl:id>GAZ:00139752</oboInOwl:id>
        <rdfs:label>Hero Bay</rdfs:label>
    </owl:NamedIndividual>
    


    <!-- http://purl.obolibrary.org/obo/GAZ_00139753 -->

    <owl:NamedIndividual rdf:about="http://purl.obolibrary.org/obo/GAZ_00139753">
        <obo:RO_0001025 rdf:resource="http://purl.obolibrary.org/obo/GAZ_00140059"/>
        <obo:IAO_0000115>A bay lying between Cape Shirreff and Essex Point on the north side of Livingston Island, in the South Shetland Islands.</obo:IAO_0000115>
        <oboInOwl:hasOBONamespace>GAZ</oboInOwl:hasOBONamespace>
        <oboInOwl:id>GAZ:00139753</oboInOwl:id>
        <rdfs:label>Barclay Bay</rdfs:label>
    </owl:NamedIndividual>
    


    <!-- http://purl.obolibrary.org/obo/GAZ_00139754 -->

    <owl:NamedIndividual rdf:about="http://purl.obolibrary.org/obo/GAZ_00139754">
        <obo:RO_0001025 rdf:resource="http://purl.obolibrary.org/obo/GAZ_00139750"/>
        <obo:IAO_0000115>The ice-covered heights of elevation 340m extending 6km in N-S direction in central and eastern Ioannes Paulus II Peninsula, Livingston Island, Antarctica. They are linked to Snow Peak to the SE by two saddles separated by the small ice dome of Casanovas Peak.</obo:IAO_0000115>
        <oboInOwl:hasOBONamespace>GAZ</oboInOwl:hasOBONamespace>
        <oboInOwl:id>GAZ:00139754</oboInOwl:id>
        <rdfs:label>Oryahovo Heights</rdfs:label>
    </owl:NamedIndividual>
    


    <!-- http://purl.obolibrary.org/obo/GAZ_00139755 -->

    <owl:NamedIndividual rdf:about="http://purl.obolibrary.org/obo/GAZ_00139755">
        <obo:RO_0001025 rdf:resource="http://purl.obolibrary.org/obo/GAZ_00139750"/>
        <obo:IAO_0000115>The ice dome rising to 325 m at the base of Ioannes Paulus II Peninsula on Livingston Island, South Shetland Islands.</obo:IAO_0000115>
        <oboInOwl:hasOBONamespace>GAZ</oboInOwl:hasOBONamespace>
        <oboInOwl:id>GAZ:00139755</oboInOwl:id>
        <rdfs:label>Casanovas Peak</rdfs:label>
    </owl:NamedIndividual>
    


    <!-- http://purl.obolibrary.org/obo/GAZ_00139769 -->

    <owl:NamedIndividual rdf:about="http://purl.obolibrary.org/obo/GAZ_00139769">
        <obo:RO_0001025 rdf:resource="http://purl.obolibrary.org/obo/GAZ_00139225"/>
        <obo:IAO_0000115>A glacially eroded basin of the Brunt Ice Shelf and partially of the Stancomb-Willis Glacier.</obo:IAO_0000115>
        <oboInOwl:hasOBONamespace>GAZ</oboInOwl:hasOBONamespace>
        <oboInOwl:id>GAZ:00139769</oboInOwl:id>
        <rdfs:label>Brunt Basin</rdfs:label>
    </owl:NamedIndividual>
    


    <!-- http://purl.obolibrary.org/obo/GAZ_00139774 -->

    <owl:NamedIndividual rdf:about="http://purl.obolibrary.org/obo/GAZ_00139774">
        <obo:RO_0001025 rdf:resource="http://purl.obolibrary.org/obo/GAZ_00141556"/>
        <obo:IAO_0000115>A bay between Fisher Island and Vollmer Island, along the coast of Marie Byrd Land. The Sulzberger Bay indents the front of the Sulzberger Ice Shelf.</obo:IAO_0000115>
        <oboInOwl:hasOBONamespace>GAZ</oboInOwl:hasOBONamespace>
        <oboInOwl:id>GAZ:00139774</oboInOwl:id>
        <rdfs:label>Sulzberger Bay</rdfs:label>
    </owl:NamedIndividual>
    


    <!-- http://purl.obolibrary.org/obo/GAZ_00139775 -->

    <owl:NamedIndividual rdf:about="http://purl.obolibrary.org/obo/GAZ_00139775">
        <obo:RO_0001025 rdf:resource="http://purl.obolibrary.org/obo/GAZ_00141556"/>
        <obo:IAO_0000115>An ice shelf about137 km long and 80 km wide bordering the coast of Marie Byrd Land between Edward VII Peninsula and Guest Peninsula.</obo:IAO_0000115>
        <oboInOwl:hasOBONamespace>GAZ</oboInOwl:hasOBONamespace>
        <oboInOwl:id>GAZ:00139775</oboInOwl:id>
        <rdfs:label>Sulzberger Ice Shelf</rdfs:label>
    </owl:NamedIndividual>
    


    <!-- http://purl.obolibrary.org/obo/GAZ_00139776 -->

    <owl:NamedIndividual rdf:about="http://purl.obolibrary.org/obo/GAZ_00139776">
        <obo:RO_0001025 rdf:resource="http://purl.obolibrary.org/obo/GAZ_00141556"/>
        <obo:IAO_0000115>An ice-covered island 11 km long, lying just North of Edward VII Peninsula where it marks the Western side of the entrance to Sulzberger Bay.</obo:IAO_0000115>
        <oboInOwl:hasOBONamespace>GAZ</oboInOwl:hasOBONamespace>
        <oboInOwl:id>GAZ:00139776</oboInOwl:id>
        <rdfs:label>Fisher Island</rdfs:label>
    </owl:NamedIndividual>
    


    <!-- http://purl.obolibrary.org/obo/GAZ_00139777 -->

    <owl:NamedIndividual rdf:about="http://purl.obolibrary.org/obo/GAZ_00139777">
        <obo:RO_0001025 rdf:resource="http://purl.obolibrary.org/obo/GAZ_00141643"/>
        <obo:IAO_0000115>An ice-covered island 11 mi long, lying along the edge of Sulzberger Ice Shelf, 7 mi NW of Cronenwett Island.</obo:IAO_0000115>
        <oboInOwl:hasOBONamespace>GAZ</oboInOwl:hasOBONamespace>
        <oboInOwl:id>GAZ:00139777</oboInOwl:id>
        <rdfs:label>Vollmer Island</rdfs:label>
    </owl:NamedIndividual>
    


    <!-- http://purl.obolibrary.org/obo/GAZ_00139778 -->

    <owl:NamedIndividual rdf:about="http://purl.obolibrary.org/obo/GAZ_00139778">
        <obo:RO_0001025 rdf:resource="http://purl.obolibrary.org/obo/GAZ_00011769"/>
        <obo:IAO_0000115>A bay on the Ross Ice Shelf of Antarctica at its juncture with Edward VII Peninsula.</obo:IAO_0000115>
        <oboInOwl:hasOBONamespace>GAZ</oboInOwl:hasOBONamespace>
        <oboInOwl:id>GAZ:00139778</oboInOwl:id>
        <rdfs:label>Okuma Bay</rdfs:label>
    </owl:NamedIndividual>
    


    <!-- http://purl.obolibrary.org/obo/GAZ_00139801 -->

    <owl:NamedIndividual rdf:about="http://purl.obolibrary.org/obo/GAZ_00139801">
        <obo:RO_0001025 rdf:resource="http://purl.obolibrary.org/obo/GAZ_00007329"/>
        <obo:IAO_0000115>A roughly rectangular ice-covered peninsula forming the northeast extremity of Livingston Island, Antarctica. It is bounded by Hero Bay to the northwest, by Moon Bay to the coutheast, and by McFarlane Strait to the northeast.</obo:IAO_0000115>
        <oboInOwl:hasOBONamespace>GAZ</oboInOwl:hasOBONamespace>
        <oboInOwl:id>GAZ:00139801</oboInOwl:id>
        <rdfs:label>Varna Peninsula</rdfs:label>
    </owl:NamedIndividual>
    


    <!-- http://purl.obolibrary.org/obo/GAZ_00139802 -->

    <owl:NamedIndividual rdf:about="http://purl.obolibrary.org/obo/GAZ_00139802">
        <rdf:type rdf:resource="http://purl.obolibrary.org/obo/ENVO_00000305"/>
        <obo:RO_0001025 rdf:resource="http://purl.obolibrary.org/obo/GAZ_00139801"/>
        <obo:IAO_0000115>A headland forming the northeast tip of Livingston Island in the South Shetland Islands.</obo:IAO_0000115>
        <oboInOwl:hasOBONamespace>GAZ</oboInOwl:hasOBONamespace>
        <oboInOwl:id>GAZ:00139802</oboInOwl:id>
        <rdfs:label>Williams Point</rdfs:label>
    </owl:NamedIndividual>
    


    <!-- http://purl.obolibrary.org/obo/GAZ_00139803 -->

    <owl:NamedIndividual rdf:about="http://purl.obolibrary.org/obo/GAZ_00139803">
        <obo:RO_0001025 rdf:resource="http://purl.obolibrary.org/obo/GAZ_00139801"/>
        <obo:IAO_0000115>Ice-covered heights rising to 604 m on Varna Peninsula, eastern Livingston Island, Antarctica. The feature is approximately 8 km long, trending west-southwest to east-northeast towards Inott Point. The summit, Miziya Peak, is located 4.2 km north-northeast of Leslie Hill and 9.25 km north by east of Mount Bowles. The heights feature Samuel Peak 1.8 km east-southeast of Miziya Peak, and Sharp Peak at their east-northeast extremity.</obo:IAO_0000115>
        <oboInOwl:hasOBONamespace>GAZ</oboInOwl:hasOBONamespace>
        <oboInOwl:id>GAZ:00139803</oboInOwl:id>
        <rdfs:label>Vidin Heights</rdfs:label>
    </owl:NamedIndividual>
    


    <!-- http://purl.obolibrary.org/obo/GAZ_00139804 -->

    <owl:NamedIndividual rdf:about="http://purl.obolibrary.org/obo/GAZ_00139804">
        <rdf:type rdf:resource="http://purl.obolibrary.org/obo/ENVO_00000305"/>
        <obo:RO_0001025 rdf:resource="http://purl.obolibrary.org/obo/GAZ_00139801"/>
        <obo:IAO_0000115>A headland 1.6 km north-northeast of Edinburgh Hill on the east coast of Livingston Island, South Shetland Islands.</obo:IAO_0000115>
        <oboInOwl:hasOBONamespace>GAZ</oboInOwl:hasOBONamespace>
        <oboInOwl:id>GAZ:00139804</oboInOwl:id>
        <rdfs:label>Inott Point</rdfs:label>
    </owl:NamedIndividual>
    


    <!-- http://purl.obolibrary.org/obo/GAZ_00139805 -->

    <owl:NamedIndividual rdf:about="http://purl.obolibrary.org/obo/GAZ_00139805">
        <obo:RO_0001025 rdf:resource="http://purl.obolibrary.org/obo/GAZ_00139801"/>
        <obo:IAO_0000115>The northwest coast of the Varna Peninsula on Livingston Island in the South Shetland Islands, Antarctica.</obo:IAO_0000115>
        <oboInOwl:hasOBONamespace>GAZ</oboInOwl:hasOBONamespace>
        <oboInOwl:id>GAZ:00139805</oboInOwl:id>
        <rdfs:label>Bezmer Point</rdfs:label>
    </owl:NamedIndividual>
    


    <!-- http://purl.obolibrary.org/obo/GAZ_00139806 -->

    <owl:NamedIndividual rdf:about="http://purl.obolibrary.org/obo/GAZ_00139806">
        <obo:RO_0001025 rdf:resource="http://purl.obolibrary.org/obo/GAZ_00007329"/>
        <obo:IAO_0000115>A ridge of elevation 330 m extending 1.5 km in S-N direction near Siddons Point on the Hero Bay coast of Livingston Island, Antarctica.</obo:IAO_0000115>
        <oboInOwl:hasOBONamespace>GAZ</oboInOwl:hasOBONamespace>
        <oboInOwl:id>GAZ:00139806</oboInOwl:id>
        <rdfs:label>Teres Ridge</rdfs:label>
    </owl:NamedIndividual>
    


    <!-- http://purl.obolibrary.org/obo/GAZ_00139807 -->

    <owl:NamedIndividual rdf:about="http://purl.obolibrary.org/obo/GAZ_00139807">
        <rdf:type rdf:resource="http://purl.obolibrary.org/obo/ENVO_00000305"/>
        <obo:RO_0001025 rdf:resource="http://purl.obolibrary.org/obo/GAZ_00139801"/>
        <obo:IAO_0000115>A headland on the NW coast of Varna Peninsula featuring a conspicuous rock near its tip, situated 2.6 km northeast of Bezmer Point, 6.4 km southwest of Williams Point and 12.8 km east-northeast of Siddons Point.</obo:IAO_0000115>
        <oboInOwl:hasOBONamespace>GAZ</oboInOwl:hasOBONamespace>
        <oboInOwl:id>GAZ:00139807</oboInOwl:id>
        <rdfs:label>Kotis Point</rdfs:label>
    </owl:NamedIndividual>
    


    <!-- http://purl.obolibrary.org/obo/GAZ_00139808 -->

    <owl:NamedIndividual rdf:about="http://purl.obolibrary.org/obo/GAZ_00139808">
        <obo:RO_0001025 rdf:resource="http://purl.obolibrary.org/obo/GAZ_00007329"/>
        <obo:IAO_0000115>A headland projecting into the middle of the head of Hero Bay on the north coast of Livingston Island, in the South Shetland Islands.</obo:IAO_0000115>
        <oboInOwl:hasOBONamespace>GAZ</oboInOwl:hasOBONamespace>
        <oboInOwl:id>GAZ:00139808</oboInOwl:id>
        <rdfs:label>Siddons Point</rdfs:label>
    </owl:NamedIndividual>
    


    <!-- http://purl.obolibrary.org/obo/GAZ_00139809 -->

    <owl:NamedIndividual rdf:about="http://purl.obolibrary.org/obo/GAZ_00139809">
        <obo:RO_0001025 rdf:resource="http://purl.obolibrary.org/obo/GAZ_00139806"/>
        <obo:IAO_0000115>A rocky point on the coast of Hero Bay, Livingston Island, formed by an offshoot of Teres Ridge.</obo:IAO_0000115>
        <oboInOwl:hasOBONamespace>GAZ</oboInOwl:hasOBONamespace>
        <oboInOwl:id>GAZ:00139809</oboInOwl:id>
        <rdfs:label>Melta Point</rdfs:label>
    </owl:NamedIndividual>
    


    <!-- http://purl.obolibrary.org/obo/GAZ_00139810 -->

    <owl:NamedIndividual rdf:about="http://purl.obolibrary.org/obo/GAZ_00139810">
        <obo:RO_0001025 rdf:resource="http://purl.obolibrary.org/obo/GAZ_00140059"/>
        <obo:IAO_0000115>A 7 mi wide bay, which recedes 4 mi between Edinburgh Hill and Renier Point, on the east side of Livingston Island, in the South Shetland Islands.</obo:IAO_0000115>
        <oboInOwl:hasOBONamespace>GAZ</oboInOwl:hasOBONamespace>
        <oboInOwl:id>GAZ:00139810</oboInOwl:id>
        <rdfs:label>Moon Bay</rdfs:label>
    </owl:NamedIndividual>
    


    <!-- http://purl.obolibrary.org/obo/GAZ_00139811 -->

    <owl:NamedIndividual rdf:about="http://purl.obolibrary.org/obo/GAZ_00139811">
        <obo:RO_0001025 rdf:resource="http://purl.obolibrary.org/obo/GAZ_00140059"/>
        <obo:IAO_0000115>The strait lying between Greenwich and Livingston Island, in the South Shetland Islands.</obo:IAO_0000115>
        <oboInOwl:hasOBONamespace>GAZ</oboInOwl:hasOBONamespace>
        <oboInOwl:id>GAZ:00139811</oboInOwl:id>
        <rdfs:label>McFarlane Strait</rdfs:label>
    </owl:NamedIndividual>
    


    <!-- http://purl.obolibrary.org/obo/GAZ_00139812 -->

    <owl:NamedIndividual rdf:about="http://purl.obolibrary.org/obo/GAZ_00139812">
        <obo:RO_0001025 rdf:resource="http://purl.obolibrary.org/obo/GAZ_00139803"/>
        <obo:IAO_0000115>A glacier on Livingston Island draining the southeastern slopes of Vidin Heights into Moon Bay between Edinburgh Hill and Helis Nunatak.</obo:IAO_0000115>
        <oboInOwl:hasOBONamespace>GAZ</oboInOwl:hasOBONamespace>
        <oboInOwl:id>GAZ:00139812</oboInOwl:id>
        <rdfs:label>Debelt Glacier</rdfs:label>
    </owl:NamedIndividual>
    


    <!-- http://purl.obolibrary.org/obo/GAZ_00139813 -->

    <owl:NamedIndividual rdf:about="http://purl.obolibrary.org/obo/GAZ_00139813">
        <obo:RO_0001025 rdf:resource="http://purl.obolibrary.org/obo/GAZ_00139803"/>
        <obo:IAO_0000115>A crown-shaped rocky peak of elevation 340 m in Vidin Heights, Livingston Island.</obo:IAO_0000115>
        <oboInOwl:hasOBONamespace>GAZ</oboInOwl:hasOBONamespace>
        <oboInOwl:id>GAZ:00139813</oboInOwl:id>
        <rdfs:label>Helis Nunatak</rdfs:label>
    </owl:NamedIndividual>
    


    <!-- http://purl.obolibrary.org/obo/GAZ_00139814 -->

    <owl:NamedIndividual rdf:about="http://purl.obolibrary.org/obo/GAZ_00139814">
        <obo:RO_0001025 rdf:resource="http://purl.obolibrary.org/obo/GAZ_00045074"/>
        <obo:IAO_0000115>An ice-covered island, 16 km long and 10 km wide, marked by rock exposures along its north and east sides, lying off Davis Peninsula in the Shackleton Ice Shelf.</obo:IAO_0000115>
        <oboInOwl:hasOBONamespace>GAZ</oboInOwl:hasOBONamespace>
        <oboInOwl:id>GAZ:00139814</oboInOwl:id>
        <rdfs:label>David Island</rdfs:label>
    </owl:NamedIndividual>
    


    <!-- http://purl.obolibrary.org/obo/GAZ_00139833 -->

    <owl:NamedIndividual rdf:about="http://purl.obolibrary.org/obo/GAZ_00139833">
        <obo:RO_0001025 rdf:resource="http://purl.obolibrary.org/obo/GAZ_00002625"/>
        <obo:IAO_0000115>A mountain outlet glacier that projects 11-12 km into McMurdo Sound from the Ross Island coastline near Cape Evans, Antarctica. The glacier tongue varies in thickness from 50 m at the snout to 300 m at the point where it is grounded on the shoreline.</obo:IAO_0000115>
        <oboInOwl:hasOBONamespace>GAZ</oboInOwl:hasOBONamespace>
        <oboInOwl:id>GAZ:00139833</oboInOwl:id>
        <rdfs:label>Erebus Ice Tongue</rdfs:label>
    </owl:NamedIndividual>
    


    <!-- http://purl.obolibrary.org/obo/GAZ_00139849 -->

    <owl:NamedIndividual rdf:about="http://purl.obolibrary.org/obo/GAZ_00139849">
        <obo:RO_0001025 rdf:resource="http://purl.obolibrary.org/obo/GAZ_00009523"/>
        <obo:IAO_0000115>A small island immediately W of the S end of Powell Island in the South Orkney Islands.</obo:IAO_0000115>
        <oboInOwl:hasOBONamespace>GAZ</oboInOwl:hasOBONamespace>
        <oboInOwl:id>GAZ:00139849</oboInOwl:id>
        <rdfs:label>Christoffersen Island</rdfs:label>
    </owl:NamedIndividual>
    


    <!-- http://purl.obolibrary.org/obo/GAZ_00139851 -->

    <owl:NamedIndividual rdf:about="http://purl.obolibrary.org/obo/GAZ_00139851">
        <obo:RO_0001025 rdf:resource="http://purl.obolibrary.org/obo/GAZ_00051499"/>
        <obo:IAO_0000115>An ice-filled embayment about 90 miles wide indenting the coast of Antarctica between Cape Goodenough and Cape Morse.</obo:IAO_0000115>
        <oboInOwl:hasOBONamespace>GAZ</oboInOwl:hasOBONamespace>
        <oboInOwl:id>GAZ:00139851</oboInOwl:id>
        <rdfs:label>Porpoise Bay</rdfs:label>
    </owl:NamedIndividual>
    


    <!-- http://purl.obolibrary.org/obo/GAZ_00139854 -->

    <owl:NamedIndividual rdf:about="http://purl.obolibrary.org/obo/GAZ_00139854">
        <obo:RO_0001025 rdf:resource="http://purl.obolibrary.org/obo/GAZ_00051499"/>
        <obo:IAO_0000115>An undersea canyon located about 300 miles from Porpoise Bay; it is one of the largest canyons in the Wilkes Land continental margin.</obo:IAO_0000115>
        <oboInOwl:hasOBONamespace>GAZ</oboInOwl:hasOBONamespace>
        <oboInOwl:id>GAZ:00139854</oboInOwl:id>
        <rdfs:label>Porpoise Canyon</rdfs:label>
    </owl:NamedIndividual>
    


    <!-- http://purl.obolibrary.org/obo/GAZ_00139855 -->

    <owl:NamedIndividual rdf:about="http://purl.obolibrary.org/obo/GAZ_00139855">
        <obo:RO_0001025 rdf:resource="http://purl.obolibrary.org/obo/GAZ_00051499"/>
        <obo:IAO_0000115>An undersea basin, located close to Porpoise Bay.</obo:IAO_0000115>
        <oboInOwl:hasOBONamespace>GAZ</oboInOwl:hasOBONamespace>
        <oboInOwl:id>GAZ:00139855</oboInOwl:id>
        <rdfs:label>Porpoise Basin</rdfs:label>
    </owl:NamedIndividual>
    


    <!-- http://purl.obolibrary.org/obo/GAZ_00139865 -->

    <owl:NamedIndividual rdf:about="http://purl.obolibrary.org/obo/GAZ_00139865">
        <obo:RO_0001025 rdf:resource="http://purl.obolibrary.org/obo/GAZ_00004045"/>
        <obo:IAO_0000115>A large, ice-filled inlet at the southwest side of Bowman Peninsula, on the east coast of Palmer Land.</obo:IAO_0000115>
        <oboInOwl:hasOBONamespace>GAZ</oboInOwl:hasOBONamespace>
        <oboInOwl:id>GAZ:00139865</oboInOwl:id>
        <rdfs:label>Gardner Inlet</rdfs:label>
    </owl:NamedIndividual>
    


    <!-- http://purl.obolibrary.org/obo/GAZ_00139892 -->

    <owl:NamedIndividual rdf:about="http://purl.obolibrary.org/obo/GAZ_00139892">
        <obo:RO_0001025 rdf:resource="http://purl.obolibrary.org/obo/GAZ_00023304"/>
        <obo:IAO_0000115>A bay about 60 mi long in the western Ross Sea, extending along the coast of Victoria Land from Cape Sibbald to Coulman Island.</obo:IAO_0000115>
        <oboInOwl:hasOBONamespace>GAZ</oboInOwl:hasOBONamespace>
        <oboInOwl:id>GAZ:00139892</oboInOwl:id>
        <rdfs:label>Lady Newnes Bay</rdfs:label>
    </owl:NamedIndividual>
    


    <!-- http://purl.obolibrary.org/obo/GAZ_00139950 -->

    <owl:NamedIndividual rdf:about="http://purl.obolibrary.org/obo/GAZ_00139950">
        <obo:RO_0001025 rdf:resource="http://purl.obolibrary.org/obo/GAZ_00141552"/>
        <obo:IAO_0000115>A fjord which is 10 miles long in an east-west direction and 5 miles wide, between Red Rock Ridge and Roman Four Promontory on the west coast of Graham Land, Antarctica.</obo:IAO_0000115>
        <oboInOwl:hasOBONamespace>GAZ</oboInOwl:hasOBONamespace>
        <oboInOwl:id>GAZ:00139950</oboInOwl:id>
        <rdfs:label>Neny Fjord</rdfs:label>
    </owl:NamedIndividual>
    


    <!-- http://purl.obolibrary.org/obo/GAZ_00139956 -->

    <owl:NamedIndividual rdf:about="http://purl.obolibrary.org/obo/GAZ_00139956">
        <obo:RO_0001025 rdf:resource="http://purl.obolibrary.org/obo/GAZ_00014084"/>
        <obo:IAO_0000115>A sound, 40 km long in a north-south direction and averaging 16 km wide, lying between the east-central portion of Adelaide Island and the south portion of Arrowsmith Peninsula, Graham Land.</obo:IAO_0000115>
        <oboInOwl:hasOBONamespace>GAZ</oboInOwl:hasOBONamespace>
        <oboInOwl:id>GAZ:00139956</oboInOwl:id>
        <rdfs:label>Laubeuf Fjord</rdfs:label>
    </owl:NamedIndividual>
    


    <!-- http://purl.obolibrary.org/obo/GAZ_00139957 -->

    <owl:NamedIndividual rdf:about="http://purl.obolibrary.org/obo/GAZ_00139957">
        <obo:RO_0001025 rdf:resource="http://purl.obolibrary.org/obo/GAZ_00045034"/>
        <obo:IAO_0000115>A fjord about 21 km long in the northeast part of Amundsen Bay, just south of Mount Riiser-Larsen.</obo:IAO_0000115>
        <oboInOwl:hasOBONamespace>GAZ</oboInOwl:hasOBONamespace>
        <oboInOwl:id>GAZ:00139957</oboInOwl:id>
        <rdfs:label>Adams Fjord</rdfs:label>
    </owl:NamedIndividual>
    


    <!-- http://purl.obolibrary.org/obo/GAZ_00139958 -->

    <owl:NamedIndividual rdf:about="http://purl.obolibrary.org/obo/GAZ_00139958">
        <obo:RO_0001025 rdf:resource="http://purl.obolibrary.org/obo/GAZ_00141552"/>
        <obo:IAO_0000115>A bay in Antarctica. It is nine miles wide at its mouth and indents five miles between Red Rock Ridge and Bertrand Ice Piedmont along the west coast of Graham Land.</obo:IAO_0000115>
        <oboInOwl:hasOBONamespace>GAZ</oboInOwl:hasOBONamespace>
        <oboInOwl:id>GAZ:00139958</oboInOwl:id>
        <rdfs:label>Rymill Bay</rdfs:label>
    </owl:NamedIndividual>
    


    <!-- http://purl.obolibrary.org/obo/GAZ_00139960 -->

    <owl:NamedIndividual rdf:about="http://purl.obolibrary.org/obo/GAZ_00139960">
        <obo:RO_0001025 rdf:resource="http://purl.obolibrary.org/obo/GAZ_00141552"/>
        <obo:IAO_0000115>A bay, 15 miles wide at its mouth and indenting 10 miles, entered between Bertrand Ice Piedmont and Cape Berteaux along the W coast of Graham Land, Antarctica.</obo:IAO_0000115>
        <oboInOwl:hasOBONamespace>GAZ</oboInOwl:hasOBONamespace>
        <oboInOwl:id>GAZ:00139960</oboInOwl:id>
        <rdfs:label>Mikkelsen Bay</rdfs:label>
    </owl:NamedIndividual>
    


    <!-- http://purl.obolibrary.org/obo/GAZ_00139963 -->

    <owl:NamedIndividual rdf:about="http://purl.obolibrary.org/obo/GAZ_00139963">
        <obo:RO_0001025 rdf:resource="http://purl.obolibrary.org/obo/GAZ_00051499"/>
        <obo:IAO_0000115>A sheltered bay formed by the junction of the western side of the Mertz Glacier Tongue and the mainland. Cape De la Motte marks the western entrance point.</obo:IAO_0000115>
        <oboInOwl:hasOBONamespace>GAZ</oboInOwl:hasOBONamespace>
        <oboInOwl:id>GAZ:00139963</oboInOwl:id>
        <rdfs:label>Buchanan Bay</rdfs:label>
    </owl:NamedIndividual>
    


    <!-- http://purl.obolibrary.org/obo/GAZ_00139966 -->

    <owl:NamedIndividual rdf:about="http://purl.obolibrary.org/obo/GAZ_00139966">
        <obo:RO_0001025 rdf:resource="http://purl.obolibrary.org/obo/GAZ_00051499"/>
        <obo:IAO_0000115>A bay about 16 mi wide indenting the coast between Garnet Point and Cape De la Motte.</obo:IAO_0000115>
        <oboInOwl:hasOBONamespace>GAZ</oboInOwl:hasOBONamespace>
        <oboInOwl:id>GAZ:00139966</oboInOwl:id>
        <rdfs:label>Watt Bay</rdfs:label>
    </owl:NamedIndividual>
    


    <!-- http://purl.obolibrary.org/obo/GAZ_00139968 -->

    <owl:NamedIndividual rdf:about="http://purl.obolibrary.org/obo/GAZ_00139968">
        <obo:RO_0001025 rdf:resource="http://purl.obolibrary.org/obo/GAZ_00051499"/>
        <obo:IAO_0000115>A narrow ice shelf, about 193 km long, which fringes Sabrina Coast between Totten Glacier and Paulding Bay. Dalton Iceberg Tongue extends north from the east part of the shelf.</obo:IAO_0000115>
        <oboInOwl:hasOBONamespace>GAZ</oboInOwl:hasOBONamespace>
        <oboInOwl:id>GAZ:00139968</oboInOwl:id>
        <rdfs:label>Moscow University Ice Shelf</rdfs:label>
    </owl:NamedIndividual>
    


    <!-- http://purl.obolibrary.org/obo/GAZ_00139971 -->

    <owl:NamedIndividual rdf:about="http://purl.obolibrary.org/obo/GAZ_00139971">
        <obo:RO_0001025 rdf:resource="http://purl.obolibrary.org/obo/GAZ_00139968"/>
        <obo:IAO_0000115>A large iceberg tongue that extends seaward from the eastern part of Moscow University Ice Shelf.</obo:IAO_0000115>
        <oboInOwl:hasOBONamespace>GAZ</oboInOwl:hasOBONamespace>
        <oboInOwl:id>GAZ:00139971</oboInOwl:id>
        <rdfs:label>Dalton Iceberg Tongue</rdfs:label>
    </owl:NamedIndividual>
    


    <!-- http://purl.obolibrary.org/obo/GAZ_00139972 -->

    <owl:NamedIndividual rdf:about="http://purl.obolibrary.org/obo/GAZ_00139972">
        <obo:RO_0001025 rdf:resource="http://purl.obolibrary.org/obo/GAZ_00051499"/>
        <obo:IAO_0000115>A bay along the coast of Antarctica just west of Clark Point. The outer portions of the bay are bounded by the Moscow University Ice Shelf and the Voyeykov Ice Shelf.</obo:IAO_0000115>
        <oboInOwl:hasOBONamespace>GAZ</oboInOwl:hasOBONamespace>
        <oboInOwl:id>GAZ:00139972</oboInOwl:id>
        <rdfs:label>Paulding Bay</rdfs:label>
    </owl:NamedIndividual>
    


    <!-- http://purl.obolibrary.org/obo/GAZ_00139973 -->

    <owl:NamedIndividual rdf:about="http://purl.obolibrary.org/obo/GAZ_00139973">
        <obo:RO_0001025 rdf:resource="http://purl.obolibrary.org/obo/GAZ_00051499"/>
        <obo:IAO_0000115>An ice shelf fringing the coast between Paulding Bay and Cape Goodenough.</obo:IAO_0000115>
        <oboInOwl:hasOBONamespace>GAZ</oboInOwl:hasOBONamespace>
        <oboInOwl:id>GAZ:00139973</oboInOwl:id>
        <rdfs:label>Voyeykov Ice Shelf</rdfs:label>
    </owl:NamedIndividual>
    


    <!-- http://purl.obolibrary.org/obo/GAZ_00139974 -->

    <owl:NamedIndividual rdf:about="http://purl.obolibrary.org/obo/GAZ_00139974">
        <obo:RO_0001025 rdf:resource="http://purl.obolibrary.org/obo/GAZ_00017735"/>
        <obo:IAO_0000115>Ice-covered heights rising to over 500 m in the NW part of Greenwich Island. Extending 10 km in NW-SE direction, and 7 km in NE-SW direction. Featuring Mount Plymouth in the E, Crutch Peaks in the NW, Lloyd Hill in the SW, and Malamir Knoll in the SE.</obo:IAO_0000115>
        <oboInOwl:hasOBONamespace>GAZ</oboInOwl:hasOBONamespace>
        <oboInOwl:id>GAZ:00139974</oboInOwl:id>
        <rdfs:label>Dryanovo Heights</rdfs:label>
    </owl:NamedIndividual>
    


    <!-- http://purl.obolibrary.org/obo/GAZ_00139975 -->

    <owl:NamedIndividual rdf:about="http://purl.obolibrary.org/obo/GAZ_00139975">
        <obo:RO_0001025 rdf:resource="http://purl.obolibrary.org/obo/GAZ_00139974"/>
        <obo:IAO_0000115>A partly ice-free ridge of elevation 240 m in Dryanovo Heights, Greenwich Island, Antarctica.</obo:IAO_0000115>
        <oboInOwl:hasOBONamespace>GAZ</oboInOwl:hasOBONamespace>
        <oboInOwl:id>GAZ:00139975</oboInOwl:id>
        <rdfs:label>Tile Ridge</rdfs:label>
    </owl:NamedIndividual>
    


    <!-- http://purl.obolibrary.org/obo/GAZ_00139976 -->

    <owl:NamedIndividual rdf:about="http://purl.obolibrary.org/obo/GAZ_00139976">
        <obo:RO_0001025 rdf:resource="http://purl.obolibrary.org/obo/GAZ_00017735"/>
        <obo:IAO_0000115>A glacier situated E and S of Lloyd Hill, and W of Tile Ridge, Greenwich Island, Antarctica. It drains southwards into McFarlane Strait between Telerig Nunatak and Triangle Point and extends 5 km in the E-W direction, and 4 km in the N-S direction.</obo:IAO_0000115>
        <oboInOwl:hasOBONamespace>GAZ</oboInOwl:hasOBONamespace>
        <oboInOwl:id>GAZ:00139976</oboInOwl:id>
        <rdfs:label>Murgash Glacier</rdfs:label>
    </owl:NamedIndividual>
    


    <!-- http://purl.obolibrary.org/obo/GAZ_00139977 -->

    <owl:NamedIndividual rdf:about="http://purl.obolibrary.org/obo/GAZ_00139977">
        <obo:RO_0001025 rdf:resource="http://purl.obolibrary.org/obo/GAZ_00139974"/>
        <obo:IAO_0000115>A rocky peak of elevation 170 m projecting from the ice cap of Greenwich Island, Antarctica in the SW extremity of Dryanovo Heights.</obo:IAO_0000115>
        <oboInOwl:hasOBONamespace>GAZ</oboInOwl:hasOBONamespace>
        <oboInOwl:id>GAZ:00139977</oboInOwl:id>
        <rdfs:label>Telerig Nunatak</rdfs:label>
    </owl:NamedIndividual>
    


    <!-- http://purl.obolibrary.org/obo/GAZ_00139981 -->

    <owl:NamedIndividual rdf:about="http://purl.obolibrary.org/obo/GAZ_00139981">
        <obo:RO_0001025 rdf:resource="http://purl.obolibrary.org/obo/GAZ_00051499"/>
        <obo:IAO_0000115>A seaward exension of the Ninnis Glacier.</obo:IAO_0000115>
        <oboInOwl:hasOBONamespace>GAZ</oboInOwl:hasOBONamespace>
        <oboInOwl:id>GAZ:00139981</oboInOwl:id>
        <rdfs:label>Ninnis Glacier Tongue</rdfs:label>
    </owl:NamedIndividual>
    


    <!-- http://purl.obolibrary.org/obo/GAZ_00139990 -->

    <owl:NamedIndividual rdf:about="http://purl.obolibrary.org/obo/GAZ_00139990">
        <obo:RO_0001025 rdf:resource="http://purl.obolibrary.org/obo/GAZ_00045057"/>
        <obo:IAO_0000115>A coastal embayment between Cape Dovers and Avalanche Rocks in Antarctica.</obo:IAO_0000115>
        <oboInOwl:hasOBONamespace>GAZ</oboInOwl:hasOBONamespace>
        <oboInOwl:id>GAZ:00139990</oboInOwl:id>
        <rdfs:label>Bay of Winds</rdfs:label>
    </owl:NamedIndividual>
    


    <!-- http://purl.obolibrary.org/obo/GAZ_00140000 -->

    <owl:NamedIndividual rdf:about="http://purl.obolibrary.org/obo/GAZ_00140000">
        <obo:RO_0001025 rdf:resource="http://purl.obolibrary.org/obo/GAZ_00004045"/>
        <obo:IAO_0000115>A bay about 7 mi wide in the western part of Luitpold Coast. This bay receives the flow of the Schweitzer Glacier and Lerchenfeld Glacier.</obo:IAO_0000115>
        <oboInOwl:hasOBONamespace>GAZ</oboInOwl:hasOBONamespace>
        <oboInOwl:id>GAZ:00140000</oboInOwl:id>
        <rdfs:label>Vahsel Bay</rdfs:label>
    </owl:NamedIndividual>
    


    <!-- http://purl.obolibrary.org/obo/GAZ_00140004 -->

    <owl:NamedIndividual rdf:about="http://purl.obolibrary.org/obo/GAZ_00140004">
        <obo:RO_0001025 rdf:resource="http://purl.obolibrary.org/obo/GAZ_00014085"/>
        <obo:IAO_0000115>A bay about 65 km long and 50 km wide, into which flows the ice of the Pine Island Glacier at the southeast extremity of the Amundsen Sea.</obo:IAO_0000115>
        <oboInOwl:hasOBONamespace>GAZ</oboInOwl:hasOBONamespace>
        <oboInOwl:id>GAZ:00140004</oboInOwl:id>
        <rdfs:label>Pine Island Bay</rdfs:label>
    </owl:NamedIndividual>
    


    <!-- http://purl.obolibrary.org/obo/GAZ_00140005 -->

    <owl:NamedIndividual rdf:about="http://purl.obolibrary.org/obo/GAZ_00140005">
        <obo:RO_0001025 rdf:resource="http://purl.obolibrary.org/obo/GAZ_00007329"/>
        <obo:IAO_0000115>A glacier located to the east of Peshev Ridge, to the south of Silistra Knoll and to the southwest of Serdica Peak in Livingston Island. The glacier flows southeastward into the Bransfield Strait between Vazov Point and Aytos Point.</obo:IAO_0000115>
        <oboInOwl:hasOBONamespace>GAZ</oboInOwl:hasOBONamespace>
        <oboInOwl:id>GAZ:00140005</oboInOwl:id>
        <rdfs:label>Boyana Glacier</rdfs:label>
    </owl:NamedIndividual>
    


    <!-- http://purl.obolibrary.org/obo/GAZ_00140006 -->

    <owl:NamedIndividual rdf:about="http://purl.obolibrary.org/obo/GAZ_00140006">
        <obo:RO_0001025 rdf:resource="http://purl.obolibrary.org/obo/GAZ_00007329"/>
        <obo:IAO_0000115>A crescent-shaped ridge extending 2 km along the NE coast of Brunow Bay and SE of Macy Glacier, Livingston Island, Antarctica. Its E extremity is formed by the summit St. Naum Peak (620 m).</obo:IAO_0000115>
        <oboInOwl:hasOBONamespace>GAZ</oboInOwl:hasOBONamespace>
        <oboInOwl:id>GAZ:00140006</oboInOwl:id>
        <rdfs:label>Peshev Ridge</rdfs:label>
    </owl:NamedIndividual>
    


    <!-- http://purl.obolibrary.org/obo/GAZ_00140007 -->

    <owl:NamedIndividual rdf:about="http://purl.obolibrary.org/obo/GAZ_00140007">
        <obo:RO_0001025 rdf:resource="http://purl.obolibrary.org/obo/GAZ_00140059"/>
        <obo:IAO_0000115>A small bay indenting the southeast side of Livingston Island, in the South Shetland Islands.</obo:IAO_0000115>
        <oboInOwl:hasOBONamespace>GAZ</oboInOwl:hasOBONamespace>
        <oboInOwl:id>GAZ:00140007</oboInOwl:id>
        <rdfs:label>Brunow Bay</rdfs:label>
    </owl:NamedIndividual>
    


    <!-- http://purl.obolibrary.org/obo/GAZ_00140008 -->

    <owl:NamedIndividual rdf:about="http://purl.obolibrary.org/obo/GAZ_00140008">
        <obo:RO_0001025 rdf:resource="http://purl.obolibrary.org/obo/GAZ_00007329"/>
        <obo:IAO_0000115>A glacier flowing into Brunow Bay, Livingston Island, in the South Shetland Islands.</obo:IAO_0000115>
        <oboInOwl:hasOBONamespace>GAZ</oboInOwl:hasOBONamespace>
        <oboInOwl:id>GAZ:00140008</oboInOwl:id>
        <rdfs:label>Macy Glacier</rdfs:label>
    </owl:NamedIndividual>
    


    <!-- http://purl.obolibrary.org/obo/GAZ_00140009 -->

    <owl:NamedIndividual rdf:about="http://purl.obolibrary.org/obo/GAZ_00140009">
        <obo:RO_0001025 rdf:resource="http://purl.obolibrary.org/obo/GAZ_00007329"/>
        <obo:IAO_0000115>A peninsula that extends 10.5 km in the east by northeast direction towards Renier Point, Livingston Island. It is bounded by Bruix Cove and Moon Bay to the north, and Bransfield Strait to the south by southeast.</obo:IAO_0000115>
        <oboInOwl:hasOBONamespace>GAZ</oboInOwl:hasOBONamespace>
        <oboInOwl:id>GAZ:00140009</oboInOwl:id>
        <rdfs:label>Burgas Peninsula</rdfs:label>
    </owl:NamedIndividual>
    


    <!-- http://purl.obolibrary.org/obo/GAZ_00140010 -->

    <owl:NamedIndividual rdf:about="http://purl.obolibrary.org/obo/GAZ_00140010">
        <obo:RO_0001025 rdf:resource="http://purl.obolibrary.org/obo/GAZ_00140009"/>
        <obo:IAO_0000115>A glacier located on the Burgas Peninsula, eastern Livingston Island, and is bounded by Ruse Peak and Asen Peak to the north and by Kuber Peak to the west. The glacier flows southeastward into Bransfield Strait.</obo:IAO_0000115>
        <oboInOwl:hasOBONamespace>GAZ</oboInOwl:hasOBONamespace>
        <oboInOwl:id>GAZ:00140010</oboInOwl:id>
        <rdfs:label>Dobrudzha Glacier</rdfs:label>
    </owl:NamedIndividual>
    


    <!-- http://purl.obolibrary.org/obo/GAZ_00140011 -->

    <owl:NamedIndividual rdf:about="http://purl.obolibrary.org/obo/GAZ_00140011">
        <obo:RO_0001025 rdf:resource="http://purl.obolibrary.org/obo/GAZ_00007329"/>
        <obo:IAO_0000115>A glacial flow on Livingston Island. The glacier runs 8 km eastward from the Worner Gap until it empties into Moon Bay. The southern edge is bounded by the Tangra Mountains, receiving glacial influx from mountain&apos;s slopes and valleys.</obo:IAO_0000115>
        <oboInOwl:hasOBONamespace>GAZ</oboInOwl:hasOBONamespace>
        <oboInOwl:id>GAZ:00140011</oboInOwl:id>
        <rdfs:label>Huron Glacier</rdfs:label>
    </owl:NamedIndividual>
    


    <!-- http://purl.obolibrary.org/obo/GAZ_00140012 -->

    <owl:NamedIndividual rdf:about="http://purl.obolibrary.org/obo/GAZ_00140012">
        <obo:RO_0001025 rdf:resource="http://purl.obolibrary.org/obo/GAZ_00007329"/>
        <obo:IAO_0000115>The principal mountain range of Livingston Island in the South Shetland Islands, Antarctica. Tangra Mountains are 30 km long between Barnard Point and Renier Point, 8 km wide, and are bounded by Moon Bay and Huron Glacier to the north, Huntress Glacier to the northwest, False Bay to the west, and Bransfield Strait to the southeast, and is linked to Bowles Ridge by Worner Gap, and to Pliska Ridge by Nesebar Gap. The mountain is divided in three principal ridges: Friesland Ridge in the west, Levski Ridge in the centre, and Delchev Ridge in the east.</obo:IAO_0000115>
        <oboInOwl:hasOBONamespace>GAZ</oboInOwl:hasOBONamespace>
        <oboInOwl:id>GAZ:00140012</oboInOwl:id>
        <rdfs:label>Tangra Mountains</rdfs:label>
    </owl:NamedIndividual>
    


    <!-- http://purl.obolibrary.org/obo/GAZ_00140013 -->

    <owl:NamedIndividual rdf:about="http://purl.obolibrary.org/obo/GAZ_00140013">
        <obo:RO_0001025 rdf:resource="http://purl.obolibrary.org/obo/GAZ_00007329"/>
        <obo:IAO_0000115>A glacier flowing into the head of False Bay, Livingston Island, in the South Shetland Islands.</obo:IAO_0000115>
        <oboInOwl:hasOBONamespace>GAZ</oboInOwl:hasOBONamespace>
        <oboInOwl:id>GAZ:00140013</oboInOwl:id>
        <rdfs:label>Huntress Glacier</rdfs:label>
    </owl:NamedIndividual>
    


    <!-- http://purl.obolibrary.org/obo/GAZ_00140014 -->

    <owl:NamedIndividual rdf:about="http://purl.obolibrary.org/obo/GAZ_00140014">
        <obo:RO_0001025 rdf:resource="http://purl.obolibrary.org/obo/GAZ_00140059"/>
        <obo:IAO_0000115>A 4 mi long bay, which lies between Barnard Point and Miers Bluff on the south side of Livingston Island, in the South Shetland Islands.</obo:IAO_0000115>
        <oboInOwl:hasOBONamespace>GAZ</oboInOwl:hasOBONamespace>
        <oboInOwl:id>GAZ:00140014</oboInOwl:id>
        <rdfs:label>False Bay</rdfs:label>
    </owl:NamedIndividual>
    


    <!-- http://purl.obolibrary.org/obo/GAZ_00140015 -->

    <owl:NamedIndividual rdf:about="http://purl.obolibrary.org/obo/GAZ_00140015">
        <rdf:type rdf:resource="http://purl.obolibrary.org/obo/ENVO_00000305"/>
        <obo:RO_0001025 rdf:resource="http://purl.obolibrary.org/obo/GAZ_00007329"/>
        <obo:IAO_0000115>A headland which marks the southeast side of the entrance to False Bay on the south side of Livingston Island, in the South Shetland Islands.</obo:IAO_0000115>
        <oboInOwl:hasOBONamespace>GAZ</oboInOwl:hasOBONamespace>
        <oboInOwl:id>GAZ:00140015</oboInOwl:id>
        <rdfs:label>Barnard Point</rdfs:label>
    </owl:NamedIndividual>
    


    <!-- http://purl.obolibrary.org/obo/GAZ_00140016 -->

    <owl:NamedIndividual rdf:about="http://purl.obolibrary.org/obo/GAZ_00140016">
        <obo:RO_0001025 rdf:resource="http://purl.obolibrary.org/obo/GAZ_00007329"/>
        <obo:IAO_0000115>The central ridge of eastern Livingston Island. The ridge extends 6.5 km in the east-west direction and is 1.5 km wide. The summit of the ridge is Mount Bowles which rises to 822m and is located 9.77 km northwest of Great Needle Peak, 6.08 km north by west of Mount Friesland, 8.77 km east-northeast of St. Kliment Ohridski base and 9.25km south by west of Miziya Peak. Bowles Ridge is bounded by Kaliakra Glacier and Struma Glacier to the north, by Perunika Glacier to the west and southwest and by Huron Glacier to the southeast and east. It is linked to Friesland Ridge of the Tangra Mountains by Worner Gap, to Hemus Peak by Dimov Gate, and to Melnik Ridge by Yankov Gap.</obo:IAO_0000115>
        <oboInOwl:hasOBONamespace>GAZ</oboInOwl:hasOBONamespace>
        <oboInOwl:id>GAZ:00140016</oboInOwl:id>
        <rdfs:label>Bowles Ridge</rdfs:label>
    </owl:NamedIndividual>
    


    <!-- http://purl.obolibrary.org/obo/GAZ_00140017 -->

    <owl:NamedIndividual rdf:about="http://purl.obolibrary.org/obo/GAZ_00140017">
        <obo:RO_0001025 rdf:resource="http://purl.obolibrary.org/obo/GAZ_00007329"/>
        <obo:IAO_0000115>A glacier in northeastern Livingston Island, Antarctica extending 7 km in E-W direction and 8 km in N-S direction. It is bounded by Melnik Ridge and Bowles Ridge to the S, by Hemus Peak, Gurev Gap, Gleaner Heights, Elhovo Gap, Leslie Hill, Leslie Gap and Radnevo Peak to the W, Miziya Peak, Samuel Peak and Perperek Knoll to the N. The glacier drains eastwards into Moon Bay.</obo:IAO_0000115>
        <oboInOwl:hasOBONamespace>GAZ</oboInOwl:hasOBONamespace>
        <oboInOwl:id>GAZ:00140017</oboInOwl:id>
        <rdfs:label>Kaliakra Glacier</rdfs:label>
    </owl:NamedIndividual>
    


    <!-- http://purl.obolibrary.org/obo/GAZ_00140018 -->

    <owl:NamedIndividual rdf:about="http://purl.obolibrary.org/obo/GAZ_00140018">
        <obo:RO_0001025 rdf:resource="http://purl.obolibrary.org/obo/GAZ_00007329"/>
        <obo:IAO_0000115>A narrow ridge rising to 696 m in eastern Livingston Island bounded by Kaliakra Glacier to the N and W, and Struma Glacier to the S and linked to Bowles Ridge by the 575 m high Yankov Gap. The ridge is 1.9 km long in the E-W direction, featuring Sliven Peak and Etropole Peak, with the summit Melnik Peak forming its W extremity. It has partly snow-free southern slopes.</obo:IAO_0000115>
        <oboInOwl:hasOBONamespace>GAZ</oboInOwl:hasOBONamespace>
        <oboInOwl:id>GAZ:00140018</oboInOwl:id>
        <rdfs:label>Melnik Ridge</rdfs:label>
    </owl:NamedIndividual>
    


    <!-- http://purl.obolibrary.org/obo/GAZ_00140019 -->

    <owl:NamedIndividual rdf:about="http://purl.obolibrary.org/obo/GAZ_00140019">
        <obo:RO_0001025 rdf:resource="http://purl.obolibrary.org/obo/GAZ_00007329"/>
        <obo:IAO_0000115>A tributary glacier in eastern Livingston Island, Antarctica draining the area between Bowles Ridge and Melnik Ridge. The glacier is 3km long and 1.5km wide, flowing eastwards into Huron Glacier. It is bounded by Melnik Ridge to the N, Yankov Gap to the W and Bowles Ridge to the S.</obo:IAO_0000115>
        <oboInOwl:hasOBONamespace>GAZ</oboInOwl:hasOBONamespace>
        <oboInOwl:id>GAZ:00140019</oboInOwl:id>
        <rdfs:label>Struma Glacier</rdfs:label>
    </owl:NamedIndividual>
    


    <!-- http://purl.obolibrary.org/obo/GAZ_00140020 -->

    <owl:NamedIndividual rdf:about="http://purl.obolibrary.org/obo/GAZ_00140020">
        <obo:RO_0001025 rdf:resource="http://purl.obolibrary.org/obo/GAZ_00007329"/>
        <obo:IAO_0000115>An 8 km long and 2.6 km wide (average) roughly crescent-shaped glacier in eastern Livingston Island, Antarctica. Its head is bounded by Pliska Ridge to the SSW, Nesebar Gap to the S, Worner Gap to the E, and Bowles Ridge to the NNE. It drains northwestwards between Burdick Ridge and Bowles Ridge, then N of Rezen Knoll turns WSW and flows into the head of Emona Anchorage between Bulgarian Beach and Pimpirev Beach.</obo:IAO_0000115>
        <oboInOwl:hasOBONamespace>GAZ</oboInOwl:hasOBONamespace>
        <oboInOwl:id>GAZ:00140020</oboInOwl:id>
        <rdfs:label>Perunika Glacier</rdfs:label>
    </owl:NamedIndividual>
    


    <!-- http://purl.obolibrary.org/obo/GAZ_00140021 -->

    <owl:NamedIndividual rdf:about="http://purl.obolibrary.org/obo/GAZ_00140021">
        <obo:RO_0001025 rdf:resource="http://purl.obolibrary.org/obo/GAZ_00007329"/>
        <obo:IAO_0000115>A ridge rising to 773 m on Livingston Island in the South Shetland Islands. Extending for 1.9 km between Orpheus Gate in the southeast and Rezen Saddle in the northwest. Bounded by Perunika Glacier to the northeast, and Balkan Snowfield to the southwest.</obo:IAO_0000115>
        <oboInOwl:hasOBONamespace>GAZ</oboInOwl:hasOBONamespace>
        <oboInOwl:id>GAZ:00140021</oboInOwl:id>
        <rdfs:label>Burdick Ridge</rdfs:label>
    </owl:NamedIndividual>
    


    <!-- http://purl.obolibrary.org/obo/GAZ_00140022 -->

    <owl:NamedIndividual rdf:about="http://purl.obolibrary.org/obo/GAZ_00140022">
        <obo:RO_0001025 rdf:resource="http://purl.obolibrary.org/obo/GAZ_00140023"/>
        <obo:IAO_0000115>A roughly square embayment forming the head of South Bay, Livingston Island.</obo:IAO_0000115>
        <oboInOwl:hasOBONamespace>GAZ</oboInOwl:hasOBONamespace>
        <oboInOwl:id>GAZ:00140022</oboInOwl:id>
        <rdfs:label>Emona Anchorage</rdfs:label>
    </owl:NamedIndividual>
    


    <!-- http://purl.obolibrary.org/obo/GAZ_00140023 -->

    <owl:NamedIndividual rdf:about="http://purl.obolibrary.org/obo/GAZ_00140023">
        <obo:RO_0001025 rdf:resource="http://purl.obolibrary.org/obo/GAZ_00140059"/>
        <obo:IAO_0000115>A 6 mi long bay lying northwest of False Bay on the south side of Livingston Island, in the South Shetland Islands.</obo:IAO_0000115>
        <oboInOwl:hasOBONamespace>GAZ</oboInOwl:hasOBONamespace>
        <oboInOwl:id>GAZ:00140023</oboInOwl:id>
        <rdfs:label>South Bay</rdfs:label>
    </owl:NamedIndividual>
    


    <!-- http://purl.obolibrary.org/obo/GAZ_00140024 -->

    <owl:NamedIndividual rdf:about="http://purl.obolibrary.org/obo/GAZ_00140024">
        <obo:RO_0001025 rdf:resource="http://purl.obolibrary.org/obo/GAZ_00007329"/>
        <obo:IAO_0000115>An ice-covered plateau ranging from 150 to 280 m in eastern Livingston Island, Western Antarctica. It is 3 km long in southwest-northeast direction and 2 km wide. It is bounded to the south-west by Krum Rock and upper Contell Glacier, to the southeast and east by the feet of Castillo Nunatak (437 m) and Burdick Ridge and to the north by the lower course of Perunika Glacier. The field slopes gently northwestwards, its foot being bounded by the hills along Bulgarian Beach.</obo:IAO_0000115>
        <oboInOwl:hasOBONamespace>GAZ</oboInOwl:hasOBONamespace>
        <oboInOwl:id>GAZ:00140024</oboInOwl:id>
        <rdfs:label>Balkan Snowfield</rdfs:label>
    </owl:NamedIndividual>
    


    <!-- http://purl.obolibrary.org/obo/GAZ_00140025 -->

    <owl:NamedIndividual rdf:about="http://purl.obolibrary.org/obo/GAZ_00140025">
        <obo:RO_0001025 rdf:resource="http://purl.obolibrary.org/obo/GAZ_00007329"/>
        <obo:IAO_0000115>A snowfield on Livingston Island, Antarctica. It is bounded by Teres Ridge to the W, the glacial divide between the Drake Passage and Bransfield Strait to the S, Gleaner Heights, Elhovo Gap and Leslie Hill to the SE, and Leslie Gap and Vidin Heights to the E. It extends 5 km inland, and 16 km in SW-NE direction and drains into Hero Bay between Melta Point and Slab Point.</obo:IAO_0000115>
        <oboInOwl:hasOBONamespace>GAZ</oboInOwl:hasOBONamespace>
        <oboInOwl:id>GAZ:00140025</oboInOwl:id>
        <rdfs:label>Saedinenie Snowfield</rdfs:label>
    </owl:NamedIndividual>
    


    <!-- http://purl.obolibrary.org/obo/GAZ_00140026 -->

    <owl:NamedIndividual rdf:about="http://purl.obolibrary.org/obo/GAZ_00140026">
        <obo:RO_0001025 rdf:resource="http://purl.obolibrary.org/obo/GAZ_00007329"/>
        <obo:IAO_0000115>A three-peaked ridge rising to 667 m in eastern Livingston Island, Antarctica. Its central and highest peak is located 2.6 km ENE of Willan Nunatak (449 m), 1.7 km SE of Burdick Peak (773 m, summit of Burdick Ridge), 3.53 km SSW of Mount Bowles, 3.68 km WSW of Kuzman Knoll, and 3.6 km NW of Mount Friesland. The feature is 1.6 km long and 500 m wide, its axis trending due E-W, with precipitous southern slopes. It is ice covered except for segments of its easternmost peak (646 m) and is bounded to the NW by Orpheus Gate, to the N by the head of Perunika Glacier, to the E by Nesebar Gap, and to the S and W by the head of Huntress Glacier, the latter flowing 6 km southwestwards into False Bay.</obo:IAO_0000115>
        <oboInOwl:hasOBONamespace>GAZ</oboInOwl:hasOBONamespace>
        <oboInOwl:id>GAZ:00140026</oboInOwl:id>
        <rdfs:label>Pliska Ridge</rdfs:label>
    </owl:NamedIndividual>
    


    <!-- http://purl.obolibrary.org/obo/GAZ_00140027 -->

    <owl:NamedIndividual rdf:about="http://purl.obolibrary.org/obo/GAZ_00140027">
        <obo:RO_0001025 rdf:resource="http://purl.obolibrary.org/obo/GAZ_00140012"/>
        <obo:IAO_0000115>A ridge that is 15.5 km long from Botev Point in the southwest to Shipka Saddle to the northeast.</obo:IAO_0000115>
        <oboInOwl:hasOBONamespace>GAZ</oboInOwl:hasOBONamespace>
        <oboInOwl:id>GAZ:00140027</oboInOwl:id>
        <rdfs:label>Friesland Ridge</rdfs:label>
    </owl:NamedIndividual>
    


    <!-- http://purl.obolibrary.org/obo/GAZ_00140028 -->

    <owl:NamedIndividual rdf:about="http://purl.obolibrary.org/obo/GAZ_00140028">
        <obo:RO_0001025 rdf:resource="http://purl.obolibrary.org/obo/GAZ_00140012"/>
        <obo:IAO_0000115>A ridge that is 10 km long between Devin Saddle to the west and Renier Point to the east.</obo:IAO_0000115>
        <oboInOwl:hasOBONamespace>GAZ</oboInOwl:hasOBONamespace>
        <oboInOwl:id>GAZ:00140028</oboInOwl:id>
        <rdfs:label>Delchev Ridge</rdfs:label>
    </owl:NamedIndividual>
    


    <!-- http://purl.obolibrary.org/obo/GAZ_00140029 -->

    <owl:NamedIndividual rdf:about="http://purl.obolibrary.org/obo/GAZ_00140029">
        <obo:RO_0001025 rdf:resource="http://purl.obolibrary.org/obo/GAZ_00140012"/>
        <obo:IAO_0000115>A ridge that is 8 km long between Shipka Saddle to the west and Devin Saddle to the east, and 8 km wide between Cherepish Ridge to the north and Christoff Cliff to the south.</obo:IAO_0000115>
        <oboInOwl:hasOBONamespace>GAZ</oboInOwl:hasOBONamespace>
        <oboInOwl:id>GAZ:00140029</oboInOwl:id>
        <rdfs:label>Levski Ridge</rdfs:label>
    </owl:NamedIndividual>
    


    <!-- http://purl.obolibrary.org/obo/GAZ_00140030 -->

    <owl:NamedIndividual rdf:about="http://purl.obolibrary.org/obo/GAZ_00140030">
        <obo:RO_0001025 rdf:resource="http://purl.obolibrary.org/obo/GAZ_00140012"/>
        <obo:IAO_0000115>An icefall that descends towards False Bay from the circus overlooked by Simeon Peak, St. Cyril Peak and St. Methodius Peak in Friesland Ridge, Tangra Mountains, eastern Livingston Island, Antarctica.</obo:IAO_0000115>
        <oboInOwl:hasOBONamespace>GAZ</oboInOwl:hasOBONamespace>
        <oboInOwl:id>GAZ:00140030</oboInOwl:id>
        <rdfs:label>Ruen Icefall</rdfs:label>
    </owl:NamedIndividual>
    


    <!-- http://purl.obolibrary.org/obo/GAZ_00140031 -->

    <owl:NamedIndividual rdf:about="http://purl.obolibrary.org/obo/GAZ_00140031">
        <obo:RO_0001025 rdf:resource="http://purl.obolibrary.org/obo/GAZ_00007329"/>
        <obo:IAO_0000115>A peninsula that extends 9 km in the SW direction towards Barnard Point, Livingston Island, Antarctica. It is bounded by False Bay to the W, and by Brunow Bay and Bransfield Strait to the SE.</obo:IAO_0000115>
        <oboInOwl:hasOBONamespace>GAZ</oboInOwl:hasOBONamespace>
        <oboInOwl:id>GAZ:00140031</oboInOwl:id>
        <rdfs:label>Rozhen Peninsula</rdfs:label>
    </owl:NamedIndividual>
    


    <!-- http://purl.obolibrary.org/obo/GAZ_00140032 -->

    <owl:NamedIndividual rdf:about="http://purl.obolibrary.org/obo/GAZ_00140032">
        <obo:RO_0001025 rdf:resource="http://purl.obolibrary.org/obo/GAZ_00140031"/>
        <obo:IAO_0000115>A glacier situated on the Rozhen Peninsula, Livingston Island in the South Shetland Islands, Antarctica. The head of the glacier is bounded by MacKay Peak (approx. 700 m) to the southwest and Tervel Peak to the east. It flows 2 km north-northwestward to terminate at the northeast extremity of Zagore Beach.</obo:IAO_0000115>
        <oboInOwl:hasOBONamespace>GAZ</oboInOwl:hasOBONamespace>
        <oboInOwl:id>GAZ:00140032</oboInOwl:id>
        <rdfs:label>Peshtera Glacier</rdfs:label>
    </owl:NamedIndividual>
    


    <!-- http://purl.obolibrary.org/obo/GAZ_00140033 -->

    <owl:NamedIndividual rdf:about="http://purl.obolibrary.org/obo/GAZ_00140033">
        <obo:RO_0001025 rdf:resource="http://purl.obolibrary.org/obo/GAZ_00007329"/>
        <obo:IAO_0000115>A glacier lying north of Barnard Point on the south coast of Livingston Island, in the South Shetland Islands.</obo:IAO_0000115>
        <oboInOwl:hasOBONamespace>GAZ</oboInOwl:hasOBONamespace>
        <oboInOwl:id>GAZ:00140033</oboInOwl:id>
        <rdfs:label>Charity Glacier</rdfs:label>
    </owl:NamedIndividual>
    


    <!-- http://purl.obolibrary.org/obo/GAZ_00140034 -->

    <owl:NamedIndividual rdf:about="http://purl.obolibrary.org/obo/GAZ_00140034">
        <obo:RO_0001025 rdf:resource="http://purl.obolibrary.org/obo/GAZ_00140031"/>
        <obo:IAO_0000115>An ice piedmont on Rozhen Peninsula, Livingston Island, Antarctica is located E of Botev Point. It is bounded to the N by Shumen Peak, to the NW and W by Gabrovo Knoll and Veleka Ridge, and to the E by Needle Peak and flows southeastwards into Bransfield Strait.</obo:IAO_0000115>
        <oboInOwl:hasOBONamespace>GAZ</oboInOwl:hasOBONamespace>
        <oboInOwl:id>GAZ:00140034</oboInOwl:id>
        <rdfs:label>Tarnovo Ice Piedmont</rdfs:label>
    </owl:NamedIndividual>
    


    <!-- http://purl.obolibrary.org/obo/GAZ_00140035 -->

    <owl:NamedIndividual rdf:about="http://purl.obolibrary.org/obo/GAZ_00140035">
        <obo:RO_0001025 rdf:resource="http://purl.obolibrary.org/obo/GAZ_00140031"/>
        <obo:IAO_0000115>A glacier on Rozhen Peninsula, Livingston Island, Antarctica is bounded to the E by Needle Peak, to the NW by St. Cyril Peak and St. Methodius Peak, and to the SW by Shumen Peak and Yambol Peak, and flows southeastward into Bransfield Strait.</obo:IAO_0000115>
        <oboInOwl:hasOBONamespace>GAZ</oboInOwl:hasOBONamespace>
        <oboInOwl:id>GAZ:00140035</oboInOwl:id>
        <rdfs:label>Prespa Glacier</rdfs:label>
    </owl:NamedIndividual>
    


    <!-- http://purl.obolibrary.org/obo/GAZ_00140036 -->

    <owl:NamedIndividual rdf:about="http://purl.obolibrary.org/obo/GAZ_00140036">
        <obo:RO_0001025 rdf:resource="http://purl.obolibrary.org/obo/GAZ_00007329"/>
        <obo:IAO_0000115>A glacier on Livingston Island, Antarctica flows SE of the Great Needle Peak and Serdica Peak to enter Bransfield Strait between Aytos Point and M&apos;Kean Point.</obo:IAO_0000115>
        <oboInOwl:hasOBONamespace>GAZ</oboInOwl:hasOBONamespace>
        <oboInOwl:id>GAZ:00140036</oboInOwl:id>
        <rdfs:label>Srebarna Glacier</rdfs:label>
    </owl:NamedIndividual>
    


    <!-- http://purl.obolibrary.org/obo/GAZ_00140037 -->

    <owl:NamedIndividual rdf:about="http://purl.obolibrary.org/obo/GAZ_00140037">
        <obo:RO_0001025 rdf:resource="http://purl.obolibrary.org/obo/GAZ_00007329"/>
        <obo:IAO_0000115>A glacier located to the north of M&apos;Kean Point, Livingston Island and is bounded by Great Needle Peak to the W, Helmet Peak and Plovdiv Peak to the north, and Ruse Peak to the northeast. It flows southeastward into Bransfield Strait.</obo:IAO_0000115>
        <oboInOwl:hasOBONamespace>GAZ</oboInOwl:hasOBONamespace>
        <oboInOwl:id>GAZ:00140037</oboInOwl:id>
        <rdfs:label>Magura Glacier</rdfs:label>
    </owl:NamedIndividual>
    


    <!-- http://purl.obolibrary.org/obo/GAZ_00140038 -->

    <owl:NamedIndividual rdf:about="http://purl.obolibrary.org/obo/GAZ_00140038">
        <obo:RO_0001025 rdf:resource="http://purl.obolibrary.org/obo/GAZ_00140009"/>
        <obo:IAO_0000115>A glacier located on the Burgas Peninsula, Livingston Island, South Shetland Islands, Antarctica The glacier is bounded by Asen Peak and Delchev Peak to the NW, flowing southeastwards into Yantra Cove, Bransfield Strait.</obo:IAO_0000115>
        <oboInOwl:hasOBONamespace>GAZ</oboInOwl:hasOBONamespace>
        <oboInOwl:id>GAZ:00140038</oboInOwl:id>
        <rdfs:label>Ropotamo Glacier</rdfs:label>
    </owl:NamedIndividual>
    


    <!-- http://purl.obolibrary.org/obo/GAZ_00140039 -->

    <owl:NamedIndividual rdf:about="http://purl.obolibrary.org/obo/GAZ_00140039">
        <obo:RO_0001025 rdf:resource="http://purl.obolibrary.org/obo/GAZ_00140059"/>
        <obo:IAO_0000115>A 750m wide cove in the south coast of the Burgas Peninsula of Livingston Island, Antarctica. The cove is east of Asen Peak and southeast of Delchev Peak.</obo:IAO_0000115>
        <oboInOwl:hasOBONamespace>GAZ</oboInOwl:hasOBONamespace>
        <oboInOwl:id>GAZ:00140039</oboInOwl:id>
        <rdfs:label>Yantra Cove</rdfs:label>
    </owl:NamedIndividual>
    


    <!-- http://purl.obolibrary.org/obo/GAZ_00140040 -->

    <owl:NamedIndividual rdf:about="http://purl.obolibrary.org/obo/GAZ_00140040">
        <obo:RO_0001025 rdf:resource="http://purl.obolibrary.org/obo/GAZ_00140009"/>
        <obo:IAO_0000115>A glacier located on Burgas Peninsula, eastern Livingston Island, Antarctica. It is bounded by Delchev Peak and Spartacus Peak to the W, and by Yavorov Peak and Elena Peak to the N and flows southeastward into Bransfield Strait.</obo:IAO_0000115>
        <oboInOwl:hasOBONamespace>GAZ</oboInOwl:hasOBONamespace>
        <oboInOwl:id>GAZ:00140040</oboInOwl:id>
        <rdfs:label>Strandzha Glacier</rdfs:label>
    </owl:NamedIndividual>
    


    <!-- http://purl.obolibrary.org/obo/GAZ_00140041 -->

    <owl:NamedIndividual rdf:about="http://purl.obolibrary.org/obo/GAZ_00140041">
        <obo:RO_0001025 rdf:resource="http://purl.obolibrary.org/obo/GAZ_00140009"/>
        <obo:IAO_0000115>A glacier on Burgas Peninsula, Livingston Island, Antarctica bounded by Petko Voyvoda Peak to the W, Kaloyan Nunatak to the N and Shabla Knoll to the E. It flows southeastward into Bransfield Strait.</obo:IAO_0000115>
        <oboInOwl:hasOBONamespace>GAZ</oboInOwl:hasOBONamespace>
        <oboInOwl:id>GAZ:00140041</oboInOwl:id>
        <rdfs:label>Pautalia Glacier</rdfs:label>
    </owl:NamedIndividual>
    


    <!-- http://purl.obolibrary.org/obo/GAZ_00140042 -->

    <owl:NamedIndividual rdf:about="http://purl.obolibrary.org/obo/GAZ_00140042">
        <obo:RO_0001025 rdf:resource="http://purl.obolibrary.org/obo/GAZ_00140009"/>
        <obo:IAO_0000115>An ice piedmont situated on Burgas Peninsula, Livingston Island, Antarctica. The glacier drains the N slopes of Delchev Ridge E of Delchev Peak, flowing northward into Moon Bay between Rila Point and Renier Point.</obo:IAO_0000115>
        <oboInOwl:hasOBONamespace>GAZ</oboInOwl:hasOBONamespace>
        <oboInOwl:id>GAZ:00140042</oboInOwl:id>
        <rdfs:label>Sopot Ice Piedmont</rdfs:label>
    </owl:NamedIndividual>
    


    <!-- http://purl.obolibrary.org/obo/GAZ_00140043 -->

    <owl:NamedIndividual rdf:about="http://purl.obolibrary.org/obo/GAZ_00140043">
        <obo:RO_0001025 rdf:resource="http://purl.obolibrary.org/obo/GAZ_00140012"/>
        <obo:IAO_0000115>A glacier in Livingston Island, draining the north slopes of the Tangra Mountains between Helmet Peak to the west and Delchev Peak to the east. It flows northward into Bruix Cove.</obo:IAO_0000115>
        <oboInOwl:hasOBONamespace>GAZ</oboInOwl:hasOBONamespace>
        <oboInOwl:id>GAZ:00140043</oboInOwl:id>
        <rdfs:label>Iskar Glacier</rdfs:label>
    </owl:NamedIndividual>
    


    <!-- http://purl.obolibrary.org/obo/GAZ_00140044 -->

    <owl:NamedIndividual rdf:about="http://purl.obolibrary.org/obo/GAZ_00140044">
        <obo:RO_0001025 rdf:resource="http://purl.obolibrary.org/obo/GAZ_00007329"/>
        <obo:IAO_0000115>A glacier located on Livingston Island south of the glacial divide between the Drake Passage and Bransfield Strait, and draining into South Bay between Ereby Point and Memorable Beach. It extends 5 km along an east-west axis, and is 2.5 km wide.</obo:IAO_0000115>
        <oboInOwl:hasOBONamespace>GAZ</oboInOwl:hasOBONamespace>
        <oboInOwl:id>GAZ:00140044</oboInOwl:id>
        <rdfs:label>Kamchiya Glacier</rdfs:label>
    </owl:NamedIndividual>
    


    <!-- http://purl.obolibrary.org/obo/GAZ_00140045 -->

    <owl:NamedIndividual rdf:about="http://purl.obolibrary.org/obo/GAZ_00140045">
        <obo:RO_0001025 rdf:resource="http://purl.obolibrary.org/obo/GAZ_00139750"/>
        <obo:IAO_0000115>A glacier bounded by the E slopes of Oryahovo Heights, Livingston Island and draining eastwards into Hero Bay between Remetalk Point and Aguero Point. It extends 2.5 km in the E-W direction, and 1.8 km in the N-S direction.</obo:IAO_0000115>
        <oboInOwl:hasOBONamespace>GAZ</oboInOwl:hasOBONamespace>
        <oboInOwl:id>GAZ:00140045</oboInOwl:id>
        <rdfs:label>Medven Glacier</rdfs:label>
    </owl:NamedIndividual>
    


    <!-- http://purl.obolibrary.org/obo/GAZ_00140046 -->

    <owl:NamedIndividual rdf:about="http://purl.obolibrary.org/obo/GAZ_00140046">
        <obo:RO_0001025 rdf:resource="http://purl.obolibrary.org/obo/GAZ_00139803"/>
        <obo:IAO_0000115>A glacier located on Livingston Island, Antarctica and drains the SE slopes of Vidin Heights into Moon Bay between Helis Nunatak and Perperek Knoll. It extends 3.5 km in the SE-NW direction, and 2.5 km in the SW-NE direction.</obo:IAO_0000115>
        <oboInOwl:hasOBONamespace>GAZ</oboInOwl:hasOBONamespace>
        <oboInOwl:id>GAZ:00140046</oboInOwl:id>
        <rdfs:label>Panega Glacier</rdfs:label>
    </owl:NamedIndividual>
    


    <!-- http://purl.obolibrary.org/obo/GAZ_00140047 -->

    <owl:NamedIndividual rdf:about="http://purl.obolibrary.org/obo/GAZ_00140047">
        <obo:RO_0001025 rdf:resource="http://purl.obolibrary.org/obo/GAZ_00007329"/>
        <obo:IAO_0000115>A glacier on Livingston Island that drains southeastwards towards Pimpirev Beach. It is situated W of Perunika Glacier, S of Tundzha Glacier and E of Kamchiya Glacier and extends 6 km in a SE-NW direction, and 2 km in NW-SE direction. The glacier mostly terminates on the shore, on several occasions penetrating the South Bay waters.</obo:IAO_0000115>
        <oboInOwl:hasOBONamespace>GAZ</oboInOwl:hasOBONamespace>
        <oboInOwl:id>GAZ:00140047</oboInOwl:id>
        <rdfs:label>Pimpirev Glacier</rdfs:label>
    </owl:NamedIndividual>
    


    <!-- http://purl.obolibrary.org/obo/GAZ_00140048 -->

    <owl:NamedIndividual rdf:about="http://purl.obolibrary.org/obo/GAZ_00140048">
        <obo:RO_0001025 rdf:resource="http://purl.obolibrary.org/obo/GAZ_00007329"/>
        <obo:IAO_0000115>A glacier on Livingston Island in the South Shetland Islands, Antarctica extending 6 km in SE-NW direction, and 3.5 km in SW-NE direction. The glacier drains the NE slopes of Vidin Heights into Lister Cove and McFarlane Strait between Pomorie Point and Inott Point.</obo:IAO_0000115>
        <oboInOwl:hasOBONamespace>GAZ</oboInOwl:hasOBONamespace>
        <oboInOwl:id>GAZ:00140048</oboInOwl:id>
        <rdfs:label>Rose Valley Glacier</rdfs:label>
    </owl:NamedIndividual>
    


    <!-- http://purl.obolibrary.org/obo/GAZ_00140049 -->

    <owl:NamedIndividual rdf:about="http://purl.obolibrary.org/obo/GAZ_00140049">
        <obo:RO_0001025 rdf:resource="http://purl.obolibrary.org/obo/GAZ_00007329"/>
        <obo:IAO_0000115>An isolated 350m long glacier located NW of Atlantic Club Ridge and SW of Hesperides Hill, and terminating on the South Bay coast in eastern Livingston Island, Antarctica.</obo:IAO_0000115>
        <oboInOwl:hasOBONamespace>GAZ</oboInOwl:hasOBONamespace>
        <oboInOwl:id>GAZ:00140049</oboInOwl:id>
        <rdfs:label>Sea Lion Glacier</rdfs:label>
    </owl:NamedIndividual>
    


    <!-- http://purl.obolibrary.org/obo/GAZ_00140050 -->

    <owl:NamedIndividual rdf:about="http://purl.obolibrary.org/obo/GAZ_00140050">
        <obo:RO_0001025 rdf:resource="http://purl.obolibrary.org/obo/GAZ_00017735"/>
        <obo:IAO_0000115>A glacier on Greenwich Island and is bounded by Viskyar Ridge to the W, and Vratsa Peak to the NE. It extends 700m in E-W direction, and 1.6 km in N-S direction, draining southwards into Bransfield Strait E of Sartorius Point.</obo:IAO_0000115>
        <oboInOwl:hasOBONamespace>GAZ</oboInOwl:hasOBONamespace>
        <oboInOwl:id>GAZ:00140050</oboInOwl:id>
        <rdfs:label>Targovishte Glacier</rdfs:label>
    </owl:NamedIndividual>
    


    <!-- http://purl.obolibrary.org/obo/GAZ_00140051 -->

    <owl:NamedIndividual rdf:about="http://purl.obolibrary.org/obo/GAZ_00140051">
        <obo:RO_0001025 rdf:resource="http://purl.obolibrary.org/obo/GAZ_00017735"/>
        <obo:IAO_0000115>Hills that rise to over 600 m in the southeast part of Greenwich Island. They extend 12 km between Santa Cruz Point in the north east and the base of the moraine spit at the mouth of Yankee Harbour in the southwest. The heights are ice covered except for limited areas such as Oborishte Ridge, Ephraim Bluff, Viskyar Ridge and Bogdan Ridge.</obo:IAO_0000115>
        <oboInOwl:hasOBONamespace>GAZ</oboInOwl:hasOBONamespace>
        <oboInOwl:id>GAZ:00140051</oboInOwl:id>
        <rdfs:label>Breznik Heights</rdfs:label>
    </owl:NamedIndividual>
    


    <!-- http://purl.obolibrary.org/obo/GAZ_00140052 -->

    <owl:NamedIndividual rdf:about="http://purl.obolibrary.org/obo/GAZ_00140052">
        <obo:RO_0001025 rdf:resource="http://purl.obolibrary.org/obo/GAZ_00140051"/>
        <obo:IAO_0000115>A rocky ridge extending 2.5 km in north-south direction in Breznik Heights, Greenwich Island, with its southern extremity forming Sartorius Point. It is bounded by Zheravna Glacier to the west and Targovishte Glacier to the east.</obo:IAO_0000115>
        <oboInOwl:hasOBONamespace>GAZ</oboInOwl:hasOBONamespace>
        <oboInOwl:id>GAZ:00140052</oboInOwl:id>
        <rdfs:label>Viskyar Ridge</rdfs:label>
    </owl:NamedIndividual>
    


    <!-- http://purl.obolibrary.org/obo/GAZ_00140053 -->

    <owl:NamedIndividual rdf:about="http://purl.obolibrary.org/obo/GAZ_00140053">
        <obo:RO_0001025 rdf:resource="http://purl.obolibrary.org/obo/GAZ_00140051"/>
        <obo:IAO_0000115>A conspicuous rocky ridge of 440 m height forming the northeastern extremity of Breznik Heights, Greenwich Island. The ridge extends 1.3 km west from Santa Cruz Point.</obo:IAO_0000115>
        <oboInOwl:hasOBONamespace>GAZ</oboInOwl:hasOBONamespace>
        <oboInOwl:id>GAZ:00140053</oboInOwl:id>
        <rdfs:label>Bogdan Ridge</rdfs:label>
    </owl:NamedIndividual>
    


    <!-- http://purl.obolibrary.org/obo/GAZ_00140054 -->

    <owl:NamedIndividual rdf:about="http://purl.obolibrary.org/obo/GAZ_00140054">
        <obo:RO_0001025 rdf:resource="http://purl.obolibrary.org/obo/GAZ_00140051"/>
        <obo:IAO_0000115>A ridge that has an elevation of 340 m in the SW extremity of Breznik Heights, Greenwich Island, Antarctica. Extending 1.6 km along the SE coast of Yankee Harbour.</obo:IAO_0000115>
        <oboInOwl:hasOBONamespace>GAZ</oboInOwl:hasOBONamespace>
        <oboInOwl:id>GAZ:00140054</oboInOwl:id>
        <rdfs:label>Oborishte Ridge</rdfs:label>
    </owl:NamedIndividual>
    


    <!-- http://purl.obolibrary.org/obo/GAZ_00140055 -->

    <owl:NamedIndividual rdf:about="http://purl.obolibrary.org/obo/GAZ_00140055">
        <obo:RO_0001025 rdf:resource="http://purl.obolibrary.org/obo/GAZ_00139974"/>
        <obo:IAO_0000115>A glacier on Greenwich Island, Antarctica draining the N slopes of Dryanovo Heights into the Drake Passage between Crutch Peaks and the ice-free area at Aguedo Point. It extends 7 km in E-W direction, and 3.5 km in N-S direction.</obo:IAO_0000115>
        <oboInOwl:hasOBONamespace>GAZ</oboInOwl:hasOBONamespace>
        <oboInOwl:id>GAZ:00140055</oboInOwl:id>
        <rdfs:label>Teteven Glacier</rdfs:label>
    </owl:NamedIndividual>
    


    <!-- http://purl.obolibrary.org/obo/GAZ_00140056 -->

    <owl:NamedIndividual rdf:about="http://purl.obolibrary.org/obo/GAZ_00140056">
        <obo:RO_0001025 rdf:resource="http://purl.obolibrary.org/obo/GAZ_00007329"/>
        <obo:IAO_0000115>A glacier on Livingston Island, Antarctica which is bounded by Snow Peak to the west, Teres Ridge to the east and the glacial divide between the Drake Passage and Bransfield Strait to the south. The glacier extends 14 km in east-west direction and 4.5km in the north-south direction, and drains northwards into Hero Bay between Avitohol Point and Siddons Point.</obo:IAO_0000115>
        <oboInOwl:hasOBONamespace>GAZ</oboInOwl:hasOBONamespace>
        <oboInOwl:id>GAZ:00140056</oboInOwl:id>
        <rdfs:label>Tundzha Glacier</rdfs:label>
    </owl:NamedIndividual>
    


    <!-- http://purl.obolibrary.org/obo/GAZ_00140057 -->

    <owl:NamedIndividual rdf:about="http://purl.obolibrary.org/obo/GAZ_00140057">
        <obo:RO_0001025 rdf:resource="http://purl.obolibrary.org/obo/GAZ_00139750"/>
        <obo:IAO_0000115>A glacier bounded by the eastern slopes of Oryahovo Heights on Livingston Island, Antarctica. The glacier drains eastwards into Hero Bay between Aguero Point and Sandanski Point. The glacier extends 2.8km in the east-west direction and 3km in the north-south direction.</obo:IAO_0000115>
        <oboInOwl:hasOBONamespace>GAZ</oboInOwl:hasOBONamespace>
        <oboInOwl:id>GAZ:00140057</oboInOwl:id>
        <rdfs:label>Urdoviza Glacier</rdfs:label>
    </owl:NamedIndividual>
    


    <!-- http://purl.obolibrary.org/obo/GAZ_00140058 -->

    <owl:NamedIndividual rdf:about="http://purl.obolibrary.org/obo/GAZ_00140058">
        <obo:RO_0001025 rdf:resource="http://purl.obolibrary.org/obo/GAZ_00007329"/>
        <obo:IAO_0000115>A glacier on Livingston Island, Antarctica is bounded by Rotch Dome to the west, Snow Peak to the north, and Ustra Peak to the southeast. It is roughly crescent-shaped, extending 13 km in an east-west direction, and 4 km in a north-south direction and drains southwards into Walker Bay between John Beach and Hannah Point.</obo:IAO_0000115>
        <oboInOwl:hasOBONamespace>GAZ</oboInOwl:hasOBONamespace>
        <oboInOwl:id>GAZ:00140058</oboInOwl:id>
        <rdfs:label>Verila Glacier</rdfs:label>
    </owl:NamedIndividual>
    


    <!-- http://purl.obolibrary.org/obo/GAZ_00140059 -->

    <owl:NamedIndividual rdf:about="http://purl.obolibrary.org/obo/GAZ_00140059">
        <obo:RO_0001025 rdf:resource="http://purl.obolibrary.org/obo/GAZ_00000373"/>
        <oboInOwl:hasOBONamespace>GAZ</oboInOwl:hasOBONamespace>
        <oboInOwl:id>GAZ:00140059</oboInOwl:id>
        <rdfs:label>Southern Ocean coastal waters of South Shetland Islands</rdfs:label>
    </owl:NamedIndividual>
    


    <!-- http://purl.obolibrary.org/obo/GAZ_00140060 -->

    <owl:NamedIndividual rdf:about="http://purl.obolibrary.org/obo/GAZ_00140060">
        <obo:RO_0001025 rdf:resource="http://purl.obolibrary.org/obo/GAZ_00140059"/>
        <obo:IAO_0000115>A bay lying between John Beach and Hannah Point along the south coast of Livingston Island, in the South Shetland Islands.</obo:IAO_0000115>
        <oboInOwl:hasOBONamespace>GAZ</oboInOwl:hasOBONamespace>
        <oboInOwl:id>GAZ:00140060</oboInOwl:id>
        <rdfs:label>Walker Bay</rdfs:label>
    </owl:NamedIndividual>
    


    <!-- http://purl.obolibrary.org/obo/GAZ_00140064 -->

    <owl:NamedIndividual rdf:about="http://purl.obolibrary.org/obo/GAZ_00140064">
        <obo:RO_0001025 rdf:resource="http://purl.obolibrary.org/obo/GAZ_00141552"/>
        <obo:IAO_0000115>An ice-filled inlet which recedes 8 miles in a northwest direction and is some 20 miles wide at its entrance between Cape Robinson and Monnier Point, along the east coast of Graham Land.</obo:IAO_0000115>
        <oboInOwl:hasOBONamespace>GAZ</oboInOwl:hasOBONamespace>
        <oboInOwl:id>GAZ:00140064</oboInOwl:id>
        <rdfs:label>Mill Inlet</rdfs:label>
    </owl:NamedIndividual>
    


    <!-- http://purl.obolibrary.org/obo/GAZ_00140066 -->

    <owl:NamedIndividual rdf:about="http://purl.obolibrary.org/obo/GAZ_00140066">
        <obo:RO_0001025 rdf:resource="http://purl.obolibrary.org/obo/GAZ_00014140"/>
        <obo:IAO_0000115>A glacier about 3.2 km long flowing north from Thurston Island just east of Dyer Point.</obo:IAO_0000115>
        <oboInOwl:hasOBONamespace>GAZ</oboInOwl:hasOBONamespace>
        <oboInOwl:id>GAZ:00140066</oboInOwl:id>
        <rdfs:label>Acosta Glacier</rdfs:label>
    </owl:NamedIndividual>
    


    <!-- http://purl.obolibrary.org/obo/GAZ_00140090 -->

    <owl:NamedIndividual rdf:about="http://purl.obolibrary.org/obo/GAZ_00140090">
        <obo:RO_0001025 rdf:resource="http://purl.obolibrary.org/obo/GAZ_00004045"/>
        <obo:IAO_0000115>A channel bounded on the west by the Antarctic Peninsula and on the east by James Ross Island. It is about 130 km long and ranges to 24 km wide.</obo:IAO_0000115>
        <oboInOwl:hasOBONamespace>GAZ</oboInOwl:hasOBONamespace>
        <oboInOwl:id>GAZ:00140090</oboInOwl:id>
        <rdfs:label>Prince Gustav Channel</rdfs:label>
    </owl:NamedIndividual>
    


    <!-- http://purl.obolibrary.org/obo/GAZ_00140091 -->

    <owl:NamedIndividual rdf:about="http://purl.obolibrary.org/obo/GAZ_00140091">
        <obo:RO_0001025 rdf:resource="http://purl.obolibrary.org/obo/GAZ_00140090"/>
        <obo:IAO_0000115>A low, nearly ice-free island less than 1 mi long. It lies in Prince Gustav Channel, about 0.5 mi off the terminus of Aitkenhead Glacier, Trinity Peninsula.</obo:IAO_0000115>
        <oboInOwl:hasOBONamespace>GAZ</oboInOwl:hasOBONamespace>
        <oboInOwl:id>GAZ:00140091</oboInOwl:id>
        <rdfs:label>Alectoria Island</rdfs:label>
    </owl:NamedIndividual>
    


    <!-- http://purl.obolibrary.org/obo/GAZ_00140092 -->

    <owl:NamedIndividual rdf:about="http://purl.obolibrary.org/obo/GAZ_00140092">
        <obo:RO_0001025 rdf:resource="http://purl.obolibrary.org/obo/GAZ_00007425"/>
        <obo:IAO_0000115>An icefall between Stenhouse Bluff and Ullmann Spur at the head of Visca Anchorage, King George Island, in the South Shetland Islands.</obo:IAO_0000115>
        <oboInOwl:hasOBONamespace>GAZ</oboInOwl:hasOBONamespace>
        <oboInOwl:id>GAZ:00140092</oboInOwl:id>
        <rdfs:label>Ajax Icefall</rdfs:label>
    </owl:NamedIndividual>
    


    <!-- http://purl.obolibrary.org/obo/GAZ_00140102 -->

    <owl:NamedIndividual rdf:about="http://purl.obolibrary.org/obo/GAZ_00140102">
        <obo:RO_0001025 rdf:resource="http://purl.obolibrary.org/obo/GAZ_00023304"/>
        <obo:IAO_0000115>A bay along the coast of Victoria Land formed by a recession in the ice between the Oates Piedmont Glacier and Evans Piedmont Glacier.</obo:IAO_0000115>
        <oboInOwl:hasOBONamespace>GAZ</oboInOwl:hasOBONamespace>
        <oboInOwl:id>GAZ:00140102</oboInOwl:id>
        <rdfs:label>Tripp Bay</rdfs:label>
    </owl:NamedIndividual>
    


    <!-- http://purl.obolibrary.org/obo/GAZ_00140103 -->

    <owl:NamedIndividual rdf:about="http://purl.obolibrary.org/obo/GAZ_00140103">
        <obo:RO_0001025 rdf:resource="http://purl.obolibrary.org/obo/GAZ_00140102"/>
        <obo:IAO_0000115>An island in the south part of Tripp Bay along the coast of Victoria Land.</obo:IAO_0000115>
        <oboInOwl:hasOBONamespace>GAZ</oboInOwl:hasOBONamespace>
        <oboInOwl:id>GAZ:00140103</oboInOwl:id>
        <rdfs:label>Tripp Island</rdfs:label>
    </owl:NamedIndividual>
    


    <!-- http://purl.obolibrary.org/obo/GAZ_00140115 -->

    <owl:NamedIndividual rdf:about="http://purl.obolibrary.org/obo/GAZ_00140115">
        <obo:RO_0001025 rdf:resource="http://purl.obolibrary.org/obo/GAZ_00141555"/>
        <obo:IAO_0000115>A bay 6 mi wide on the coast of Enderby Land, lying 12 mi E of Freeth Bay in Alasheyev Bight.</obo:IAO_0000115>
        <oboInOwl:hasOBONamespace>GAZ</oboInOwl:hasOBONamespace>
        <oboInOwl:id>GAZ:00140115</oboInOwl:id>
        <rdfs:label>Spooner Bay</rdfs:label>
    </owl:NamedIndividual>
    


    <!-- http://purl.obolibrary.org/obo/GAZ_00140119 -->

    <owl:NamedIndividual rdf:about="http://purl.obolibrary.org/obo/GAZ_00140119">
        <obo:RO_0001025 rdf:resource="http://purl.obolibrary.org/obo/GAZ_00051499"/>
        <obo:IAO_0000115>A bay lying between Lunik Point and Cape Williams. Lillie Glacier Tongue occupies the east part of the bay.</obo:IAO_0000115>
        <oboInOwl:hasOBONamespace>GAZ</oboInOwl:hasOBONamespace>
        <oboInOwl:id>GAZ:00140119</oboInOwl:id>
        <rdfs:label>Ob&apos; Bay</rdfs:label>
    </owl:NamedIndividual>
    


    <!-- http://purl.obolibrary.org/obo/GAZ_00140129 -->

    <owl:NamedIndividual rdf:about="http://purl.obolibrary.org/obo/GAZ_00140129">
        <obo:RO_0001025 rdf:resource="http://purl.obolibrary.org/obo/GAZ_00004045"/>
        <obo:IAO_0000115>An ice-filled inlet at the terminus of Casey Glacier, between Miller Point and Cape Walcott, on the E coast of Palmer Land.</obo:IAO_0000115>
        <oboInOwl:hasOBONamespace>GAZ</oboInOwl:hasOBONamespace>
        <oboInOwl:id>GAZ:00140129</oboInOwl:id>
        <rdfs:label>Casey Inlet</rdfs:label>
    </owl:NamedIndividual>
    


    <!-- http://purl.obolibrary.org/obo/GAZ_00140134 -->

    <owl:NamedIndividual rdf:about="http://purl.obolibrary.org/obo/GAZ_00140134">
        <obo:RO_0001025 rdf:resource="http://purl.obolibrary.org/obo/GAZ_00004045"/>
        <obo:IAO_0000115>An ice-filled inlet, 36 miles long in a NW-SE direction, and some 27 miles wide at its entrance between Cape Alexander and Cape Robinson, along the east coast of Graham Land.</obo:IAO_0000115>
        <oboInOwl:hasOBONamespace>GAZ</oboInOwl:hasOBONamespace>
        <oboInOwl:id>GAZ:00140134</oboInOwl:id>
        <rdfs:label>Cabinet Inlet</rdfs:label>
    </owl:NamedIndividual>
    


    <!-- http://purl.obolibrary.org/obo/GAZ_00140140 -->

    <owl:NamedIndividual rdf:about="http://purl.obolibrary.org/obo/GAZ_00140140">
        <obo:RO_0001025 rdf:resource="http://purl.obolibrary.org/obo/GAZ_00004057"/>
        <obo:IAO_0000115>A large glacier draining that part of Ross Island between Mount Erebus and Mount Terra Nova, and flowing south into McMurdo Ice Shelf.</obo:IAO_0000115>
        <oboInOwl:hasOBONamespace>GAZ</oboInOwl:hasOBONamespace>
        <oboInOwl:id>GAZ:00140140</oboInOwl:id>
        <rdfs:label>Aurora Glacier</rdfs:label>
    </owl:NamedIndividual>
    


    <!-- http://purl.obolibrary.org/obo/GAZ_00140145 -->

    <owl:NamedIndividual rdf:about="http://purl.obolibrary.org/obo/GAZ_00140145">
        <obo:RO_0001025 rdf:resource="http://purl.obolibrary.org/obo/GAZ_00051128"/>
        <obo:IAO_0000115>A cove in southern Hanusse Bay indenting the northwest side of Arrowsmith Peninsula in Graham Land.</obo:IAO_0000115>
        <oboInOwl:hasOBONamespace>GAZ</oboInOwl:hasOBONamespace>
        <oboInOwl:id>GAZ:00140145</oboInOwl:id>
        <rdfs:label>Shumskiy Cove</rdfs:label>
    </owl:NamedIndividual>
    


    <!-- http://purl.obolibrary.org/obo/GAZ_00140146 -->

    <owl:NamedIndividual rdf:about="http://purl.obolibrary.org/obo/GAZ_00140146">
        <obo:RO_0001025 rdf:resource="http://purl.obolibrary.org/obo/GAZ_00014119"/>
        <obo:IAO_0000115>A teep glacier which descends from the west slopes of Mount Erebus and terminates on the west side of Ross Island, between Cape Barne and Cape Evans where it forms a steep ice cliff.</obo:IAO_0000115>
        <oboInOwl:hasOBONamespace>GAZ</oboInOwl:hasOBONamespace>
        <oboInOwl:id>GAZ:00140146</oboInOwl:id>
        <rdfs:label>Barne Glacier</rdfs:label>
    </owl:NamedIndividual>
    


    <!-- http://purl.obolibrary.org/obo/GAZ_00140149 -->

    <owl:NamedIndividual rdf:about="http://purl.obolibrary.org/obo/GAZ_00140149">
        <obo:RO_0001025 rdf:resource="http://purl.obolibrary.org/obo/GAZ_00023304"/>
        <obo:IAO_0000115>An ice-filled inlet at the terminus of the Skelton Glacier, along the western edge of the Ross Ice Shelf in Antarctica. The feature is about 16 km wide at the entry points between Cape Timberlake and Fishtail Point, where it is about 1500 m deep.</obo:IAO_0000115>
        <oboInOwl:hasOBONamespace>GAZ</oboInOwl:hasOBONamespace>
        <oboInOwl:id>GAZ:00140149</oboInOwl:id>
        <rdfs:label>Skelton Inlet</rdfs:label>
    </owl:NamedIndividual>
    


    <!-- http://purl.obolibrary.org/obo/GAZ_00140159 -->

    <owl:NamedIndividual rdf:about="http://purl.obolibrary.org/obo/GAZ_00140159">
        <obo:RO_0001025 rdf:resource="http://purl.obolibrary.org/obo/GAZ_00141556"/>
        <obo:IAO_0000115>An ice shelf about 35 mi wide, lying N of Siemiatkowski Glacier and the W part of Ruppert Coast, Marie Byrd Land.</obo:IAO_0000115>
        <oboInOwl:hasOBONamespace>GAZ</oboInOwl:hasOBONamespace>
        <oboInOwl:id>GAZ:00140159</oboInOwl:id>
        <rdfs:label>Nickerson Ice Shelf</rdfs:label>
    </owl:NamedIndividual>
    


    <!-- http://purl.obolibrary.org/obo/GAZ_00140164 -->

    <owl:NamedIndividual rdf:about="http://purl.obolibrary.org/obo/GAZ_00140164">
        <obo:RO_0001025 rdf:resource="http://purl.obolibrary.org/obo/GAZ_00004057"/>
        <obo:IAO_0000115>A piedmont glacier, 10 km long and 3.2 km wide, between the southwest part of Mount Bird and Micou Point, Ross Island.</obo:IAO_0000115>
        <oboInOwl:hasOBONamespace>GAZ</oboInOwl:hasOBONamespace>
        <oboInOwl:id>GAZ:00140164</oboInOwl:id>
        <rdfs:label>Endeavour Piedmont Glacier</rdfs:label>
    </owl:NamedIndividual>
    


    <!-- http://purl.obolibrary.org/obo/GAZ_00140165 -->

    <owl:NamedIndividual rdf:about="http://purl.obolibrary.org/obo/GAZ_00140165">
        <obo:RO_0001025 rdf:resource="http://purl.obolibrary.org/obo/GAZ_00014113"/>
        <obo:IAO_0000115>A broad glacier north of Mount Elder, draining southeast to the south coast of Elephant Island, South Shetland Islands. It is the main discharge glacier on the island.</obo:IAO_0000115>
        <oboInOwl:hasOBONamespace>GAZ</oboInOwl:hasOBONamespace>
        <oboInOwl:id>GAZ:00140165</oboInOwl:id>
        <rdfs:label>Endurance Glacier</rdfs:label>
    </owl:NamedIndividual>
    


    <!-- http://purl.obolibrary.org/obo/GAZ_00140175 -->

    <owl:NamedIndividual rdf:about="http://purl.obolibrary.org/obo/GAZ_00140175">
        <obo:RO_0001025 rdf:resource="http://purl.obolibrary.org/obo/GAZ_00004045"/>
        <obo:IAO_0000115>An ice-filled inlet, 8 mi wide, which recedes SW for 17 mi between Cape Boggs and Cape Sharbonneau, along the E coast of Palmer Land.</obo:IAO_0000115>
        <oboInOwl:hasOBONamespace>GAZ</oboInOwl:hasOBONamespace>
        <oboInOwl:id>GAZ:00140175</oboInOwl:id>
        <rdfs:label>Lehrke Inlet</rdfs:label>
    </owl:NamedIndividual>
    


    <!-- http://purl.obolibrary.org/obo/GAZ_00140176 -->

    <owl:NamedIndividual rdf:about="http://purl.obolibrary.org/obo/GAZ_00140176">
        <obo:RO_0001025 rdf:resource="http://purl.obolibrary.org/obo/GAZ_00004045"/>
        <obo:IAO_0000115>An island 1 mi long, lying close W of Steele Island and 10 mi NW of Cape Bryant, off the E coast of Palmer Land.</obo:IAO_0000115>
        <oboInOwl:hasOBONamespace>GAZ</oboInOwl:hasOBONamespace>
        <oboInOwl:id>GAZ:00140176</oboInOwl:id>
        <rdfs:label>Morency Island</rdfs:label>
    </owl:NamedIndividual>
    


    <!-- http://purl.obolibrary.org/obo/GAZ_00140191 -->

    <owl:NamedIndividual rdf:about="http://purl.obolibrary.org/obo/GAZ_00140191">
        <rdf:type rdf:resource="http://purl.obolibrary.org/obo/ENVO_00000032"/>
        <obo:RO_0001025 rdf:resource="http://purl.obolibrary.org/obo/GAZ_00051499"/>
        <obo:IAO_0000115>An embayment of the coastline at the terminus of Rennick Glacier. It is bounded on the west and east by Belousov Point and Stuhlinger Ice Piedmont.</obo:IAO_0000115>
        <oboInOwl:hasOBONamespace>GAZ</oboInOwl:hasOBONamespace>
        <oboInOwl:id>GAZ:00140191</oboInOwl:id>
        <rdfs:label>Rennick Bay</rdfs:label>
    </owl:NamedIndividual>
    


    <!-- http://purl.obolibrary.org/obo/GAZ_00140192 -->

    <owl:NamedIndividual rdf:about="http://purl.obolibrary.org/obo/GAZ_00140192">
        <obo:RO_0001025 rdf:resource="http://purl.obolibrary.org/obo/GAZ_00140191"/>
        <obo:IAO_0000115>A high, nearly round, ice-covered island 4.0 km long, lying in Rennick Bay just north of the terminus of Rennick Glacier.</obo:IAO_0000115>
        <oboInOwl:hasOBONamespace>GAZ</oboInOwl:hasOBONamespace>
        <oboInOwl:id>GAZ:00140192</oboInOwl:id>
        <rdfs:label>Znamenskiy Island</rdfs:label>
    </owl:NamedIndividual>
    


    <!-- http://purl.obolibrary.org/obo/GAZ_00140206 -->

    <owl:NamedIndividual rdf:about="http://purl.obolibrary.org/obo/GAZ_00140206">
        <obo:RO_0001025 rdf:resource="http://purl.obolibrary.org/obo/GAZ_00007475"/>
        <obo:IAO_0000115>AAn ice shelf about 60 km long on the south shore of Prydz Bay, between Mount Caroline Mikkelsen and Stornes Peninsula. Several glaciers, listed from southwest to northeast, nourish the ice shelf: Polar Times Glacier, Il Polo Glacier, Polarforschung Glacier, Polar Record Glacier and Polararboken Glacier.</obo:IAO_0000115>
        <oboInOwl:hasOBONamespace>GAZ</oboInOwl:hasOBONamespace>
        <oboInOwl:id>GAZ:00140206</oboInOwl:id>
        <rdfs:label>Publications Ice Shelf</rdfs:label>
    </owl:NamedIndividual>
    


    <!-- http://purl.obolibrary.org/obo/GAZ_00140213 -->

    <owl:NamedIndividual rdf:about="http://purl.obolibrary.org/obo/GAZ_00140213">
        <obo:RO_0001025 rdf:resource="http://purl.obolibrary.org/obo/GAZ_00140206"/>
        <obo:IAO_0000115>Two rock islands in the E part of Publications Ice Shelf, about 8 mi SE of the Sostrene Islands.</obo:IAO_0000115>
        <oboInOwl:hasOBONamespace>GAZ</oboInOwl:hasOBONamespace>
        <oboInOwl:id>GAZ:00140213</oboInOwl:id>
        <rdfs:label>Stein Islands</rdfs:label>
    </owl:NamedIndividual>
    


    <!-- http://purl.obolibrary.org/obo/GAZ_00140214 -->

    <owl:NamedIndividual rdf:about="http://purl.obolibrary.org/obo/GAZ_00140214">
        <obo:RO_0001025 rdf:resource="http://purl.obolibrary.org/obo/GAZ_00140206"/>
        <obo:IAO_0000115>A group of small islands and rocks that rise above the northern part of Publications Ice Shelf at the head of Prydz Bay.</obo:IAO_0000115>
        <oboInOwl:hasOBONamespace>GAZ</oboInOwl:hasOBONamespace>
        <oboInOwl:id>GAZ:00140214</oboInOwl:id>
        <rdfs:label>Sostrene Islands</rdfs:label>
    </owl:NamedIndividual>
    


    <!-- http://purl.obolibrary.org/obo/GAZ_00140215 -->

    <owl:NamedIndividual rdf:about="http://purl.obolibrary.org/obo/GAZ_00140215">
        <obo:RO_0001025 rdf:resource="http://purl.obolibrary.org/obo/GAZ_00004381"/>
        <obo:IAO_0000115>A glacier flowing northeast from the central highlands of Anvers Island between the Achaean and Trojan Ranges into Lapeyrere Bay, in the Palmer Archipelago.</obo:IAO_0000115>
        <oboInOwl:hasOBONamespace>GAZ</oboInOwl:hasOBONamespace>
        <oboInOwl:id>GAZ:00140215</oboInOwl:id>
        <rdfs:label>Iliad Glacier</rdfs:label>
    </owl:NamedIndividual>
    


    <!-- http://purl.obolibrary.org/obo/GAZ_00140216 -->

    <owl:NamedIndividual rdf:about="http://purl.obolibrary.org/obo/GAZ_00140216">
        <obo:RO_0001025 rdf:resource="http://purl.obolibrary.org/obo/GAZ_00045077"/>
        <obo:IAO_0000115>A glacier flowing northwest into Gin Cove, James Ross Island.</obo:IAO_0000115>
        <oboInOwl:hasOBONamespace>GAZ</oboInOwl:hasOBONamespace>
        <oboInOwl:id>GAZ:00140216</oboInOwl:id>
        <rdfs:label>Ineson Glacier</rdfs:label>
    </owl:NamedIndividual>
    


    <!-- http://purl.obolibrary.org/obo/GAZ_00140217 -->

    <owl:NamedIndividual rdf:about="http://purl.obolibrary.org/obo/GAZ_00140217">
        <obo:RO_0001025 rdf:resource="http://purl.obolibrary.org/obo/GAZ_00004045"/>
        <obo:IAO_0000115>A cove indenting the northwest coast of James Ross Island to the north of Tumbledown Cliffs.</obo:IAO_0000115>
        <oboInOwl:hasOBONamespace>GAZ</oboInOwl:hasOBONamespace>
        <oboInOwl:id>GAZ:00140217</oboInOwl:id>
        <rdfs:label>Gin Cove</rdfs:label>
    </owl:NamedIndividual>
    


    <!-- http://purl.obolibrary.org/obo/GAZ_00140234 -->

    <owl:NamedIndividual rdf:about="http://purl.obolibrary.org/obo/GAZ_00140234">
        <obo:RO_0001025 rdf:resource="http://purl.obolibrary.org/obo/GAZ_00014140"/>
        <obo:IAO_0000115>A small glacier flowing south from Thurston Island between Cox and Hale Glaciers.</obo:IAO_0000115>
        <oboInOwl:hasOBONamespace>GAZ</oboInOwl:hasOBONamespace>
        <oboInOwl:id>GAZ:00140234</oboInOwl:id>
        <rdfs:label>Isbrecht Glacier</rdfs:label>
    </owl:NamedIndividual>
    


    <!-- http://purl.obolibrary.org/obo/GAZ_00140235 -->

    <owl:NamedIndividual rdf:about="http://purl.obolibrary.org/obo/GAZ_00140235">
        <obo:RO_0001025 rdf:resource="http://purl.obolibrary.org/obo/GAZ_00014140"/>
        <obo:IAO_0000115>A small glacier immediately E of Rochray Glacier on Thurston Island, flowing S to Abbot Ice Shelf in Peacock Sound.</obo:IAO_0000115>
        <oboInOwl:hasOBONamespace>GAZ</oboInOwl:hasOBONamespace>
        <oboInOwl:id>GAZ:00140235</oboInOwl:id>
        <rdfs:label>Cox Glacier</rdfs:label>
    </owl:NamedIndividual>
    


    <!-- http://purl.obolibrary.org/obo/GAZ_00140236 -->

    <owl:NamedIndividual rdf:about="http://purl.obolibrary.org/obo/GAZ_00140236">
        <obo:RO_0001025 rdf:resource="http://purl.obolibrary.org/obo/GAZ_00014140"/>
        <obo:IAO_0000115>A glacier about 5 mi long, located just E of Hendersin Knob on Thurston Island and flowing S to Abbot Ice Shelf in Peacock Sound.</obo:IAO_0000115>
        <oboInOwl:hasOBONamespace>GAZ</oboInOwl:hasOBONamespace>
        <oboInOwl:id>GAZ:00140236</oboInOwl:id>
        <rdfs:label>Rochray Glacier</rdfs:label>
    </owl:NamedIndividual>
    


    <!-- http://purl.obolibrary.org/obo/GAZ_00140237 -->

    <owl:NamedIndividual rdf:about="http://purl.obolibrary.org/obo/GAZ_00140237">
        <obo:RO_0001025 rdf:resource="http://purl.obolibrary.org/obo/GAZ_00014140"/>
        <obo:IAO_0000115>A glacier about 6 mi long, located just E of Mount Simpson on Thurston Island and flowing SW to Abbot Ice Shelf in Peacock Sound.</obo:IAO_0000115>
        <oboInOwl:hasOBONamespace>GAZ</oboInOwl:hasOBONamespace>
        <oboInOwl:id>GAZ:00140237</oboInOwl:id>
        <rdfs:label>Hale Glacier</rdfs:label>
    </owl:NamedIndividual>
    


    <!-- http://purl.obolibrary.org/obo/GAZ_00140250 -->

    <owl:NamedIndividual rdf:about="http://purl.obolibrary.org/obo/GAZ_00140250">
        <obo:RO_0001025 rdf:resource="http://purl.obolibrary.org/obo/GAZ_00141555"/>
        <obo:IAO_0000115>A large bay indenting the coast of Enderby Land between Tange Promontory and Dingle Dome.</obo:IAO_0000115>
        <oboInOwl:hasOBONamespace>GAZ</oboInOwl:hasOBONamespace>
        <oboInOwl:id>GAZ:00140250</oboInOwl:id>
        <rdfs:label>Casey Bay</rdfs:label>
    </owl:NamedIndividual>
    


    <!-- http://purl.obolibrary.org/obo/GAZ_00140251 -->

    <owl:NamedIndividual rdf:about="http://purl.obolibrary.org/obo/GAZ_00140251">
        <obo:RO_0001025 rdf:resource="http://purl.obolibrary.org/obo/GAZ_00141555"/>
        <obo:IAO_0000115>A large island, mostly ice covered, in the Hannan Ice Shelf along the coast of Enderby Land.</obo:IAO_0000115>
        <oboInOwl:hasOBONamespace>GAZ</oboInOwl:hasOBONamespace>
        <oboInOwl:id>GAZ:00140251</oboInOwl:id>
        <rdfs:label>McKinnon Island</rdfs:label>
    </owl:NamedIndividual>
    


    <!-- http://purl.obolibrary.org/obo/GAZ_00140252 -->

    <owl:NamedIndividual rdf:about="http://purl.obolibrary.org/obo/GAZ_00140252">
        <obo:RO_0001025 rdf:resource="http://purl.obolibrary.org/obo/GAZ_00141555"/>
        <obo:IAO_0000115>An ice shelf 18 mi wide on the coast of Enderby Land. The ice shelf is nourished by Molle and Kichenside Glaciers and borders McKinnon Island on all but its N side.</obo:IAO_0000115>
        <oboInOwl:hasOBONamespace>GAZ</oboInOwl:hasOBONamespace>
        <oboInOwl:id>GAZ:00140252</oboInOwl:id>
        <rdfs:label>Hannan Ice Shelf</rdfs:label>
    </owl:NamedIndividual>
    


    <!-- http://purl.obolibrary.org/obo/GAZ_00140256 -->

    <owl:NamedIndividual rdf:about="http://purl.obolibrary.org/obo/GAZ_00140256">
        <obo:RO_0001025 rdf:resource="http://purl.obolibrary.org/obo/GAZ_00141555"/>
        <obo:IAO_0000115>A small ice shelf which borders the south side of Sakellari Peninsula in Enderby Land.</obo:IAO_0000115>
        <oboInOwl:hasOBONamespace>GAZ</oboInOwl:hasOBONamespace>
        <oboInOwl:id>GAZ:00140256</oboInOwl:id>
        <rdfs:label>Zubchatyy Ice Shelf</rdfs:label>
    </owl:NamedIndividual>
    


    <!-- http://purl.obolibrary.org/obo/GAZ_00140257 -->

    <owl:NamedIndividual rdf:about="http://purl.obolibrary.org/obo/GAZ_00140257">
        <obo:RO_0001025 rdf:resource="http://purl.obolibrary.org/obo/GAZ_00141555"/>
        <obo:IAO_0000115>An ice-covered island 13 miles long and 5 miles wide, lying 6 miles north of Sakellari Peninsula, Enderby Land.</obo:IAO_0000115>
        <oboInOwl:hasOBONamespace>GAZ</oboInOwl:hasOBONamespace>
        <oboInOwl:id>GAZ:00140257</oboInOwl:id>
        <rdfs:label>White Island</rdfs:label>
    </owl:NamedIndividual>
    


    <!-- http://purl.obolibrary.org/obo/GAZ_00140258 -->

    <owl:NamedIndividual rdf:about="http://purl.obolibrary.org/obo/GAZ_00140258">
        <obo:RO_0001025 rdf:resource="http://purl.obolibrary.org/obo/GAZ_00141555"/>
        <obo:IAO_0000115>A small Antarctic ice shelf located on the east side of the base of Sakellari Peninsula.</obo:IAO_0000115>
        <oboInOwl:hasOBONamespace>GAZ</oboInOwl:hasOBONamespace>
        <oboInOwl:id>GAZ:00140258</oboInOwl:id>
        <rdfs:label>Wyers Ice Shelf</rdfs:label>
    </owl:NamedIndividual>
    


    <!-- http://purl.obolibrary.org/obo/GAZ_00140260 -->

    <owl:NamedIndividual rdf:about="http://purl.obolibrary.org/obo/GAZ_00140260">
        <obo:RO_0001025 rdf:resource="http://purl.obolibrary.org/obo/GAZ_00141552"/>
        <obo:IAO_0000115>A bay 12 mi long and 6 mi wide, between Cape Garcia and Loqui Point on the W coast of Graham Land.</obo:IAO_0000115>
        <oboInOwl:hasOBONamespace>GAZ</oboInOwl:hasOBONamespace>
        <oboInOwl:id>GAZ:00140260</oboInOwl:id>
        <rdfs:label>Barilari Bay</rdfs:label>
    </owl:NamedIndividual>
    


    <!-- http://purl.obolibrary.org/obo/GAZ_00140261 -->

    <owl:NamedIndividual rdf:about="http://purl.obolibrary.org/obo/GAZ_00140261">
        <obo:RO_0001025 rdf:resource="http://purl.obolibrary.org/obo/GAZ_00023319"/>
        <obo:IAO_0000115>A confluent glacier system which flows into Marshall Bay on the south coast of Coronation Island, in the South Orkney Islands.</obo:IAO_0000115>
        <oboInOwl:hasOBONamespace>GAZ</oboInOwl:hasOBONamespace>
        <oboInOwl:id>GAZ:00140261</oboInOwl:id>
        <rdfs:label>Laws Glacier</rdfs:label>
    </owl:NamedIndividual>
    


    <!-- http://purl.obolibrary.org/obo/GAZ_00140262 -->

    <owl:NamedIndividual rdf:about="http://purl.obolibrary.org/obo/GAZ_00140262">
        <obo:RO_0001025 rdf:resource="http://purl.obolibrary.org/obo/GAZ_00141024"/>
        <obo:IAO_0000115>A bay 2 mi wide, lying between Capes Vik and Hansen on the S side of Coronation Island, in the South Orkney Islands.</obo:IAO_0000115>
        <oboInOwl:hasOBONamespace>GAZ</oboInOwl:hasOBONamespace>
        <oboInOwl:id>GAZ:00140262</oboInOwl:id>
        <rdfs:label>Marshall Bay</rdfs:label>
    </owl:NamedIndividual>
    


    <!-- http://purl.obolibrary.org/obo/GAZ_00140267 -->

    <owl:NamedIndividual rdf:about="http://purl.obolibrary.org/obo/GAZ_00140267">
        <obo:RO_0001025 rdf:resource="http://purl.obolibrary.org/obo/GAZ_00023304"/>
        <obo:IAO_0000115>A broad glacier tongue extending eastward from the Mawson Glacier into the Ross Sea in Antarctica.</obo:IAO_0000115>
        <oboInOwl:hasOBONamespace>GAZ</oboInOwl:hasOBONamespace>
        <oboInOwl:id>GAZ:00140267</oboInOwl:id>
        <rdfs:label>Nordenskjold Ice Tongue</rdfs:label>
    </owl:NamedIndividual>
    


    <!-- http://purl.obolibrary.org/obo/GAZ_00140270 -->

    <owl:NamedIndividual rdf:about="http://purl.obolibrary.org/obo/GAZ_00140270">
        <obo:RO_0001025 rdf:resource="http://purl.obolibrary.org/obo/GAZ_00009523"/>
        <obo:IAO_0000115>A precipitous island 1.6 km south of Point Rae, off the south coast of Laurie Island in the South Orkney Islands.</obo:IAO_0000115>
        <oboInOwl:hasOBONamespace>GAZ</oboInOwl:hasOBONamespace>
        <oboInOwl:id>GAZ:00140270</oboInOwl:id>
        <rdfs:label>Ailsa Craig</rdfs:label>
    </owl:NamedIndividual>
    


    <!-- http://purl.obolibrary.org/obo/GAZ_00140271 -->

    <owl:NamedIndividual rdf:about="http://purl.obolibrary.org/obo/GAZ_00140271">
        <obo:RO_0001025 rdf:resource="http://purl.obolibrary.org/obo/GAZ_00009005"/>
        <obo:IAO_0000115>A British research station of Signy Island.</obo:IAO_0000115>
        <oboInOwl:hasOBONamespace>GAZ</oboInOwl:hasOBONamespace>
        <oboInOwl:id>GAZ:00140271</oboInOwl:id>
        <rdfs:label>Signy Research Station</rdfs:label>
    </owl:NamedIndividual>
    


    <!-- http://purl.obolibrary.org/obo/GAZ_00140299 -->

    <owl:NamedIndividual rdf:about="http://purl.obolibrary.org/obo/GAZ_00140299">
        <obo:RO_0001025 rdf:resource="http://purl.obolibrary.org/obo/GAZ_00140355"/>
        <obo:IAO_0000115>A western lobe of the Mount Bird Icecap, descending steeply into Wohlschlag Bay 1.6 km south of Cinder Hill on Ross Island.</obo:IAO_0000115>
        <oboInOwl:hasOBONamespace>GAZ</oboInOwl:hasOBONamespace>
        <oboInOwl:id>GAZ:00140299</oboInOwl:id>
        <rdfs:label>Quaternary Icefall</rdfs:label>
    </owl:NamedIndividual>
    


    <!-- http://purl.obolibrary.org/obo/GAZ_00140300 -->

    <owl:NamedIndividual rdf:about="http://purl.obolibrary.org/obo/GAZ_00140300">
        <obo:RO_0001025 rdf:resource="http://purl.obolibrary.org/obo/GAZ_00004057"/>
        <obo:IAO_0000115>A stratovolcano, 1,765 m, standing about 11 km south of Cape Bird, the north extremity of Ross Island.</obo:IAO_0000115>
        <oboInOwl:hasOBONamespace>GAZ</oboInOwl:hasOBONamespace>
        <oboInOwl:id>GAZ:00140300</oboInOwl:id>
        <rdfs:label>Mount Bird</rdfs:label>
    </owl:NamedIndividual>
    


    <!-- http://purl.obolibrary.org/obo/GAZ_00140301 -->

    <owl:NamedIndividual rdf:about="http://purl.obolibrary.org/obo/GAZ_00140301">
        <obo:RO_0001025 rdf:resource="http://purl.obolibrary.org/obo/GAZ_00017735"/>
        <obo:IAO_0000115>A glacier flowing north into the sea west of Canto Point in north Greenwich Island, South Shetland Islands.</obo:IAO_0000115>
        <oboInOwl:hasOBONamespace>GAZ</oboInOwl:hasOBONamespace>
        <oboInOwl:id>GAZ:00140301</oboInOwl:id>
        <rdfs:label>Quito Glacier</rdfs:label>
    </owl:NamedIndividual>
    


    <!-- http://purl.obolibrary.org/obo/GAZ_00140302 -->

    <owl:NamedIndividual rdf:about="http://purl.obolibrary.org/obo/GAZ_00140302">
        <rdf:type rdf:resource="http://purl.obolibrary.org/obo/ENVO_00000305"/>
        <obo:RO_0001025 rdf:resource="http://purl.obolibrary.org/obo/GAZ_00017735"/>
        <obo:IAO_0000115>A headland forming the NW side of the entrance to Discovery Bay, Greenwich Island, in the South Shetland Islands.</obo:IAO_0000115>
        <oboInOwl:hasOBONamespace>GAZ</oboInOwl:hasOBONamespace>
        <oboInOwl:id>GAZ:00140302</oboInOwl:id>
        <rdfs:label>Canto Point</rdfs:label>
    </owl:NamedIndividual>
    


    <!-- http://purl.obolibrary.org/obo/GAZ_00140310 -->

    <owl:NamedIndividual rdf:about="http://purl.obolibrary.org/obo/GAZ_00140310">
        <obo:RO_0001025 rdf:resource="http://purl.obolibrary.org/obo/GAZ_00139422"/>
        <obo:IAO_0000115>A bay about 32 km in extent, entered between Edward VIII Plateau and the Oygarden Group.</obo:IAO_0000115>
        <oboInOwl:hasOBONamespace>GAZ</oboInOwl:hasOBONamespace>
        <oboInOwl:id>GAZ:00140310</oboInOwl:id>
        <rdfs:label>Edward VIII Bay</rdfs:label>
    </owl:NamedIndividual>
    


    <!-- http://purl.obolibrary.org/obo/GAZ_00140311 -->

    <owl:NamedIndividual rdf:about="http://purl.obolibrary.org/obo/GAZ_00140311">
        <obo:RO_0001025 rdf:resource="http://purl.obolibrary.org/obo/GAZ_00140310"/>
        <obo:IAO_0000115>An ice shelf occupying the head of Edward VII Bay.</obo:IAO_0000115>
        <oboInOwl:hasOBONamespace>GAZ</oboInOwl:hasOBONamespace>
        <oboInOwl:id>GAZ:00140311</oboInOwl:id>
        <rdfs:label>Edward VIII Ice Shelf</rdfs:label>
    </owl:NamedIndividual>
    


    <!-- http://purl.obolibrary.org/obo/GAZ_00140312 -->

    <owl:NamedIndividual rdf:about="http://purl.obolibrary.org/obo/GAZ_00140312">
        <obo:RO_0001025 rdf:resource="http://purl.obolibrary.org/obo/GAZ_00141555"/>
        <obo:IAO_0000115>A shallow coastal indentation, 7 miles wide and receding only 2 miles, located 9 miles west of Cape Davis at the northwest side of Edward VIII Plateau, in Antarctica.</obo:IAO_0000115>
        <oboInOwl:hasOBONamespace>GAZ</oboInOwl:hasOBONamespace>
        <oboInOwl:id>GAZ:00140312</oboInOwl:id>
        <rdfs:label>Magnet Bay</rdfs:label>
    </owl:NamedIndividual>
    


    <!-- http://purl.obolibrary.org/obo/GAZ_00140313 -->

    <owl:NamedIndividual rdf:about="http://purl.obolibrary.org/obo/GAZ_00140313">
        <obo:RO_0001025 rdf:resource="http://purl.obolibrary.org/obo/GAZ_00139422"/>
        <obo:IAO_0000115>A coastal embayment at the W side of William Scoresby Archipelago, 5 mi long and 3.5 mi wide, with shores marked by steep rock headlands and snow-free hills rising to 210 m. The practical limits of the bay are extended 4 mi northward from the coast by island groups located along its E and W margin.</obo:IAO_0000115>
        <oboInOwl:hasOBONamespace>GAZ</oboInOwl:hasOBONamespace>
        <oboInOwl:id>GAZ:00140313</oboInOwl:id>
        <rdfs:label>William Scoresby Bay</rdfs:label>
    </owl:NamedIndividual>
    


    <!-- http://purl.obolibrary.org/obo/GAZ_00140314 -->

    <owl:NamedIndividual rdf:about="http://purl.obolibrary.org/obo/GAZ_00140314">
        <obo:RO_0001025 rdf:resource="http://purl.obolibrary.org/obo/GAZ_00139422"/>
        <obo:IAO_0000115>A rocky island, 4 mi long and rising to 140 m, with a prominent cove indenting the N side, situated 2 mi N of Law Promontory and 1 mi W of Havstein Island.</obo:IAO_0000115>
        <oboInOwl:hasOBONamespace>GAZ</oboInOwl:hasOBONamespace>
        <oboInOwl:id>GAZ:00140314</oboInOwl:id>
        <rdfs:label>Broka Island</rdfs:label>
    </owl:NamedIndividual>
    


    <!-- http://purl.obolibrary.org/obo/GAZ_00140315 -->

    <owl:NamedIndividual rdf:about="http://purl.obolibrary.org/obo/GAZ_00140315">
        <obo:RO_0001025 rdf:resource="http://purl.obolibrary.org/obo/GAZ_00139422"/>
        <obo:IAO_0000115>A rocky island, 3 mi long and 2 mi wide, situated 1.5 mi N of Law Promontory and 1 mi E of Broka Island.</obo:IAO_0000115>
        <oboInOwl:hasOBONamespace>GAZ</oboInOwl:hasOBONamespace>
        <oboInOwl:id>GAZ:00140315</oboInOwl:id>
        <rdfs:label>Havstein Island</rdfs:label>
    </owl:NamedIndividual>
    


    <!-- http://purl.obolibrary.org/obo/GAZ_00140320 -->

    <owl:NamedIndividual rdf:about="http://purl.obolibrary.org/obo/GAZ_00140320">
        <obo:RO_0001025 rdf:resource="http://purl.obolibrary.org/obo/GAZ_00139422"/>
        <obo:IAO_0000115>A coastal rock outcrop which rises to 120 m on the W side of Hoseason Glacier, 14 mi SE of Edward VIII Bay.</obo:IAO_0000115>
        <oboInOwl:hasOBONamespace>GAZ</oboInOwl:hasOBONamespace>
        <oboInOwl:id>GAZ:00140320</oboInOwl:id>
        <rdfs:label>West Stack</rdfs:label>
    </owl:NamedIndividual>
    


    <!-- http://purl.obolibrary.org/obo/GAZ_00140321 -->

    <owl:NamedIndividual rdf:about="http://purl.obolibrary.org/obo/GAZ_00140321">
        <obo:RO_0001025 rdf:resource="http://purl.obolibrary.org/obo/GAZ_00139422"/>
        <obo:IAO_0000115>A coastal rock outcrop which rises to 60 m on the E side of Hoseason Glacier, 16 mi SE of Edward VIII Bay.</obo:IAO_0000115>
        <oboInOwl:hasOBONamespace>GAZ</oboInOwl:hasOBONamespace>
        <oboInOwl:id>GAZ:00140321</oboInOwl:id>
        <rdfs:label>East Stack</rdfs:label>
    </owl:NamedIndividual>
    


    <!-- http://purl.obolibrary.org/obo/GAZ_00140325 -->

    <owl:NamedIndividual rdf:about="http://purl.obolibrary.org/obo/GAZ_00140325">
        <obo:RO_0001025 rdf:resource="http://purl.obolibrary.org/obo/GAZ_00141552"/>
        <obo:IAO_0000115>A bay about 10 mi wide between Cape Kater and Cape Kjellman along the W coast of Graham Land.</obo:IAO_0000115>
        <oboInOwl:hasOBONamespace>GAZ</oboInOwl:hasOBONamespace>
        <oboInOwl:id>GAZ:00140325</oboInOwl:id>
        <rdfs:label>Charcot Bay</rdfs:label>
    </owl:NamedIndividual>
    


    <!-- http://purl.obolibrary.org/obo/GAZ_00140326 -->

    <owl:NamedIndividual rdf:about="http://purl.obolibrary.org/obo/GAZ_00140326">
        <obo:RO_0001025 rdf:resource="http://purl.obolibrary.org/obo/GAZ_00014084"/>
        <obo:IAO_0000115>A bay 7 mi wide lying E of Havilland Point, along the W coast of Graham Land.</obo:IAO_0000115>
        <oboInOwl:hasOBONamespace>GAZ</oboInOwl:hasOBONamespace>
        <oboInOwl:id>GAZ:00140326</oboInOwl:id>
        <rdfs:label>Lanchester Bay</rdfs:label>
    </owl:NamedIndividual>
    


    <!-- http://purl.obolibrary.org/obo/GAZ_00140327 -->

    <owl:NamedIndividual rdf:about="http://purl.obolibrary.org/obo/GAZ_00140327">
        <obo:RO_0001025 rdf:resource="http://purl.obolibrary.org/obo/GAZ_00141554"/>
        <obo:IAO_0000115>An ice shelf about 40 miles wide, fronting on the coast of Queen Maud Land northward of Giaever Ridge.</obo:IAO_0000115>
        <oboInOwl:hasOBONamespace>GAZ</oboInOwl:hasOBONamespace>
        <oboInOwl:id>GAZ:00140327</oboInOwl:id>
        <rdfs:label>Jelbart Ice Shelf</rdfs:label>
    </owl:NamedIndividual>
    


    <!-- http://purl.obolibrary.org/obo/GAZ_00140341 -->

    <owl:NamedIndividual rdf:about="http://purl.obolibrary.org/obo/GAZ_00140341">
        <obo:RO_0001025 rdf:resource="http://purl.obolibrary.org/obo/GAZ_00023301"/>
        <obo:IAO_0000115>A steep glacier 6 km long and 10 km wide, with very prominent hummocks and crevasses, flowing east between Mount Bouvier and Mount Mangin into Stonehouse Bay on the east side of Adelaide Island.</obo:IAO_0000115>
        <oboInOwl:hasOBONamespace>GAZ</oboInOwl:hasOBONamespace>
        <oboInOwl:id>GAZ:00140341</oboInOwl:id>
        <rdfs:label>Shambles Glacier</rdfs:label>
    </owl:NamedIndividual>
    


    <!-- http://purl.obolibrary.org/obo/GAZ_00140352 -->

    <owl:NamedIndividual rdf:about="http://purl.obolibrary.org/obo/GAZ_00140352">
        <obo:RO_0001025 rdf:resource="http://purl.obolibrary.org/obo/GAZ_00023301"/>
        <obo:IAO_0000115>A glacier flowing southeast from Mount Mangin into Ryder Bay, Adelaide Island.</obo:IAO_0000115>
        <oboInOwl:hasOBONamespace>GAZ</oboInOwl:hasOBONamespace>
        <oboInOwl:id>GAZ:00140352</oboInOwl:id>
        <rdfs:label>Sheldon Glacier</rdfs:label>
    </owl:NamedIndividual>
    


    <!-- http://purl.obolibrary.org/obo/GAZ_00140353 -->

    <owl:NamedIndividual rdf:about="http://purl.obolibrary.org/obo/GAZ_00140353">
        <obo:RO_0001025 rdf:resource="http://purl.obolibrary.org/obo/GAZ_00141552"/>
        <obo:IAO_0000115>A bay 6 mi wide at its mouth and indenting 4 mi, lying 5 mi E of Mount Gaudry on the SE coast of Adelaide Island. The Leonie Islands lie across the mouth of this bay.</obo:IAO_0000115>
        <oboInOwl:hasOBONamespace>GAZ</oboInOwl:hasOBONamespace>
        <oboInOwl:id>GAZ:00140353</oboInOwl:id>
        <rdfs:label>Ryder Bay</rdfs:label>
    </owl:NamedIndividual>
    


    <!-- http://purl.obolibrary.org/obo/GAZ_00140354 -->

    <owl:NamedIndividual rdf:about="http://purl.obolibrary.org/obo/GAZ_00140354">
        <obo:RO_0001025 rdf:resource="http://purl.obolibrary.org/obo/GAZ_00140355"/>
        <obo:IAO_0000115>A western lobe of the Mount Bird Icecap. It descends steeply in the valley north of Trachyte Hill and Harrison Bluff in the center of the ice-free area on the lower western slopes of Mount Bird, Ross Island.</obo:IAO_0000115>
        <oboInOwl:hasOBONamespace>GAZ</oboInOwl:hasOBONamespace>
        <oboInOwl:id>GAZ:00140354</oboInOwl:id>
        <rdfs:label>Shell Glacier</rdfs:label>
    </owl:NamedIndividual>
    


    <!-- http://purl.obolibrary.org/obo/GAZ_00140355 -->

    <owl:NamedIndividual rdf:about="http://purl.obolibrary.org/obo/GAZ_00140355">
        <obo:RO_0001025 rdf:resource="http://purl.obolibrary.org/obo/GAZ_00140300"/>
        <oboInOwl:hasOBONamespace>GAZ</oboInOwl:hasOBONamespace>
        <oboInOwl:id>GAZ:00140355</oboInOwl:id>
        <rdfs:label>Mount Bird Icecap</rdfs:label>
    </owl:NamedIndividual>
    


    <!-- http://purl.obolibrary.org/obo/GAZ_00140364 -->

    <owl:NamedIndividual rdf:about="http://purl.obolibrary.org/obo/GAZ_00140364">
        <rdf:type rdf:resource="http://purl.obolibrary.org/obo/ENVO_00000475"/>
        <obo:RO_0001025 rdf:resource="http://purl.obolibrary.org/obo/GAZ_00140365"/>
        <obo:IAO_0000115>An arm of Robertson Bay, 6 km wide, lying between Cape Wood and Birthday Point along the north coast of Victoria Land.</obo:IAO_0000115>
        <oboInOwl:hasOBONamespace>GAZ</oboInOwl:hasOBONamespace>
        <oboInOwl:id>GAZ:00140364</oboInOwl:id>
        <rdfs:label>Pressure Bay</rdfs:label>
    </owl:NamedIndividual>
    


    <!-- http://purl.obolibrary.org/obo/GAZ_00140365 -->

    <owl:NamedIndividual rdf:about="http://purl.obolibrary.org/obo/GAZ_00140365">
        <obo:RO_0001025 rdf:resource="http://purl.obolibrary.org/obo/GAZ_00051499"/>
        <obo:IAO_0000115>A large, roughly triangular bay that indents the N coast of Victoria Land between Cape Barrow and Cape Adare.</obo:IAO_0000115>
        <oboInOwl:hasOBONamespace>GAZ</oboInOwl:hasOBONamespace>
        <oboInOwl:id>GAZ:00140365</oboInOwl:id>
        <rdfs:label>Robertson Bay</rdfs:label>
    </owl:NamedIndividual>
    


    <!-- http://purl.obolibrary.org/obo/GAZ_00140366 -->

    <owl:NamedIndividual rdf:about="http://purl.obolibrary.org/obo/GAZ_00140366">
        <obo:RO_0001025 rdf:resource="http://purl.obolibrary.org/obo/GAZ_00023294"/>
        <obo:IAO_0000115>A bay comprising the narrow southernmost, or &quot;bottom,&quot; portion of Lutzow-Holm Bay, marking its head.</obo:IAO_0000115>
        <oboInOwl:hasOBONamespace>GAZ</oboInOwl:hasOBONamespace>
        <oboInOwl:id>GAZ:00140366</oboInOwl:id>
        <rdfs:label>Havsbotn</rdfs:label>
    </owl:NamedIndividual>
    


    <!-- http://purl.obolibrary.org/obo/GAZ_00140370 -->

    <owl:NamedIndividual rdf:about="http://purl.obolibrary.org/obo/GAZ_00140370">
        <obo:RO_0001025 rdf:resource="http://purl.obolibrary.org/obo/GAZ_00141552"/>
        <obo:IAO_0000115>A bay, roughly square in outline and 10 mi wide, indenting the W coast of Graham Land between Nicholl Head and Camp Point. Most of the entrance to the bay is occupied by Horseshoe Island, which limits access to a narrow southern strait opening onto Marguerite Bay and a narrower northwestern strait opening onto the mouth of Bourgeois Fjord.</obo:IAO_0000115>
        <oboInOwl:hasOBONamespace>GAZ</oboInOwl:hasOBONamespace>
        <oboInOwl:id>GAZ:00140370</oboInOwl:id>
        <rdfs:label>Square Bay</rdfs:label>
    </owl:NamedIndividual>
    


    <!-- http://purl.obolibrary.org/obo/GAZ_00140371 -->

    <owl:NamedIndividual rdf:about="http://purl.obolibrary.org/obo/GAZ_00140371">
        <obo:RO_0001025 rdf:resource="http://purl.obolibrary.org/obo/GAZ_00140370"/>
        <obo:IAO_0000115>An island 6.5 mi long and 3 mi wide occupying most of the entrance to Square Bay, along the W coast of Graham Land. Discovered and named by the BGLE under Rymill who mapped this area by land and from the air in 1936-37. Its name is indicative of the crescentic alignment of the 600 to 900 m peaks which give a comparable shape to the island.</obo:IAO_0000115>
        <oboInOwl:hasOBONamespace>GAZ</oboInOwl:hasOBONamespace>
        <oboInOwl:id>GAZ:00140371</oboInOwl:id>
        <rdfs:label>Horseshoe Island</rdfs:label>
    </owl:NamedIndividual>
    


    <!-- http://purl.obolibrary.org/obo/GAZ_00140372 -->

    <owl:NamedIndividual rdf:about="http://purl.obolibrary.org/obo/GAZ_00140372">
        <obo:RO_0001025 rdf:resource="http://purl.obolibrary.org/obo/GAZ_00140370"/>
        <obo:IAO_0000115>A bay 2.5 mi wide which indents the W side of Horseshoe Island, in the NE part of Marguerite Bay.</obo:IAO_0000115>
        <oboInOwl:hasOBONamespace>GAZ</oboInOwl:hasOBONamespace>
        <oboInOwl:id>GAZ:00140372</oboInOwl:id>
        <rdfs:label>Lystad Bay</rdfs:label>
    </owl:NamedIndividual>
    


    <!-- http://purl.obolibrary.org/obo/GAZ_00140373 -->

    <owl:NamedIndividual rdf:about="http://purl.obolibrary.org/obo/GAZ_00140373">
        <obo:RO_0001025 rdf:resource="http://purl.obolibrary.org/obo/GAZ_00140370"/>
        <obo:IAO_0000115>A cove indenting the NE side of Horseshoe Island, off Graham Land.</obo:IAO_0000115>
        <oboInOwl:hasOBONamespace>GAZ</oboInOwl:hasOBONamespace>
        <oboInOwl:id>GAZ:00140373</oboInOwl:id>
        <rdfs:label>Gaul Cove</rdfs:label>
    </owl:NamedIndividual>
    


    <!-- http://purl.obolibrary.org/obo/GAZ_00140374 -->

    <owl:NamedIndividual rdf:about="http://purl.obolibrary.org/obo/GAZ_00140374">
        <obo:RO_0001025 rdf:resource="http://purl.obolibrary.org/obo/GAZ_00140371"/>
        <obo:IAO_0000115>The largest glacier on Horseshoe Island, flowing westward into both Lystad Bay and Gaul Cove.</obo:IAO_0000115>
        <oboInOwl:hasOBONamespace>GAZ</oboInOwl:hasOBONamespace>
        <oboInOwl:id>GAZ:00140374</oboInOwl:id>
        <rdfs:label>Shoesmith Glacier</rdfs:label>
    </owl:NamedIndividual>
    


    <!-- http://purl.obolibrary.org/obo/GAZ_00140378 -->

    <owl:NamedIndividual rdf:about="http://purl.obolibrary.org/obo/GAZ_00140378">
        <obo:RO_0001025 rdf:resource="http://purl.obolibrary.org/obo/GAZ_00014088"/>
        <obo:IAO_0000115>A glacier, 19 km long and 10 km wide, flowing south into Mozart Ice Piedmont 16 km southwest of Mount Stephenson in the north part of Alexander Island.</obo:IAO_0000115>
        <oboInOwl:hasOBONamespace>GAZ</oboInOwl:hasOBONamespace>
        <oboInOwl:id>GAZ:00140378</oboInOwl:id>
        <rdfs:label>Sibelius Glacier</rdfs:label>
    </owl:NamedIndividual>
    


    <!-- http://purl.obolibrary.org/obo/GAZ_00140379 -->

    <owl:NamedIndividual rdf:about="http://purl.obolibrary.org/obo/GAZ_00140379">
        <obo:RO_0001025 rdf:resource="http://purl.obolibrary.org/obo/GAZ_00014088"/>
        <obo:IAO_0000115>An ice piedmont, 60 mi long in a NW-SE direction and 15 mi wide in its widest part, on the W coast of Alexander Island.</obo:IAO_0000115>
        <oboInOwl:hasOBONamespace>GAZ</oboInOwl:hasOBONamespace>
        <oboInOwl:id>GAZ:00140379</oboInOwl:id>
        <rdfs:label>Mozart Ice Piedmont</rdfs:label>
    </owl:NamedIndividual>
    


    <!-- http://purl.obolibrary.org/obo/GAZ_00140380 -->

    <owl:NamedIndividual rdf:about="http://purl.obolibrary.org/obo/GAZ_00140380">
        <obo:RO_0001025 rdf:resource="http://purl.obolibrary.org/obo/GAZ_00014088"/>
        <obo:IAO_0000115>A cluster of four small mountains in north-western Alexander Island, 21 km long in the northeast-southwest direction and 13 km wide.</obo:IAO_0000115>
        <oboInOwl:hasOBONamespace>GAZ</oboInOwl:hasOBONamespace>
        <oboInOwl:id>GAZ:00140380</oboInOwl:id>
        <rdfs:label>Sofia University Mountains</rdfs:label>
    </owl:NamedIndividual>
    


    <!-- http://purl.obolibrary.org/obo/GAZ_00140381 -->

    <owl:NamedIndividual rdf:about="http://purl.obolibrary.org/obo/GAZ_00140381">
        <obo:RO_0001025 rdf:resource="http://purl.obolibrary.org/obo/GAZ_00014088"/>
        <obo:IAO_0000115>A prominent mountain range, reaching about 2,800 m and extending 60 km NW-SE from Mount Bayonne to Care Heights and Mount Cupola, in north Alexander Island, Antarctica.</obo:IAO_0000115>
        <oboInOwl:hasOBONamespace>GAZ</oboInOwl:hasOBONamespace>
        <oboInOwl:id>GAZ:00140381</oboInOwl:id>
        <rdfs:label>Rouen Mountains</rdfs:label>
    </owl:NamedIndividual>
    


    <!-- http://purl.obolibrary.org/obo/GAZ_00140382 -->

    <owl:NamedIndividual rdf:about="http://purl.obolibrary.org/obo/GAZ_00140382">
        <obo:RO_0001025 rdf:resource="http://purl.obolibrary.org/obo/GAZ_00014088"/>
        <obo:IAO_0000115>Mountains forming the NW extremity of Alexander Island, extending 20 mi in an E-W direction between Cape Vostok and Russian Gap.</obo:IAO_0000115>
        <oboInOwl:hasOBONamespace>GAZ</oboInOwl:hasOBONamespace>
        <oboInOwl:id>GAZ:00140382</oboInOwl:id>
        <rdfs:label>Havre Mountains</rdfs:label>
    </owl:NamedIndividual>
    


    <!-- http://purl.obolibrary.org/obo/GAZ_00140383 -->

    <owl:NamedIndividual rdf:about="http://purl.obolibrary.org/obo/GAZ_00140383">
        <obo:RO_0001025 rdf:resource="http://purl.obolibrary.org/obo/GAZ_00014088"/>
        <obo:IAO_0000115>Uplands rising to 1,900 m, between Tufts Pass to the N and Sullivan Glacier to the S, in the N part of Alexander Island.</obo:IAO_0000115>
        <oboInOwl:hasOBONamespace>GAZ</oboInOwl:hasOBONamespace>
        <oboInOwl:id>GAZ:00140383</oboInOwl:id>
        <rdfs:label>Elgar Uplands</rdfs:label>
    </owl:NamedIndividual>
    


    <!-- http://purl.obolibrary.org/obo/GAZ_00140384 -->

    <owl:NamedIndividual rdf:about="http://purl.obolibrary.org/obo/GAZ_00140384">
        <obo:RO_0001025 rdf:resource="http://purl.obolibrary.org/obo/GAZ_00014088"/>
        <obo:IAO_0000115>A glacier flowing W into Gilbert Glacier, immediately S of Elgar Uplands in the N part of Alexander Island.</obo:IAO_0000115>
        <oboInOwl:hasOBONamespace>GAZ</oboInOwl:hasOBONamespace>
        <oboInOwl:id>GAZ:00140384</oboInOwl:id>
        <rdfs:label>Sullivan Glacier</rdfs:label>
    </owl:NamedIndividual>
    


    <!-- http://purl.obolibrary.org/obo/GAZ_00140385 -->

    <owl:NamedIndividual rdf:about="http://purl.obolibrary.org/obo/GAZ_00140385">
        <obo:RO_0001025 rdf:resource="http://purl.obolibrary.org/obo/GAZ_00014088"/>
        <obo:IAO_0000115>A glacier c. 20 mi long flowing S from Nichols Snowfield into Mozart Ice Piedmont, Alexander Island.</obo:IAO_0000115>
        <oboInOwl:hasOBONamespace>GAZ</oboInOwl:hasOBONamespace>
        <oboInOwl:id>GAZ:00140385</oboInOwl:id>
        <rdfs:label>Gilbert Glacier</rdfs:label>
    </owl:NamedIndividual>
    


    <!-- http://purl.obolibrary.org/obo/GAZ_00140386 -->

    <owl:NamedIndividual rdf:about="http://purl.obolibrary.org/obo/GAZ_00140386">
        <obo:RO_0001025 rdf:resource="http://purl.obolibrary.org/obo/GAZ_00014088"/>
        <obo:IAO_0000115>Snowfield, 22 mi long and 8 mi wide, bounded by the Rouen Mountains and Elgar Uplands to the E and Lassus Mountains to the W, in the N part of Alexander Island.</obo:IAO_0000115>
        <oboInOwl:hasOBONamespace>GAZ</oboInOwl:hasOBONamespace>
        <oboInOwl:id>GAZ:00140386</oboInOwl:id>
        <rdfs:label>Nichols Snowfield</rdfs:label>
    </owl:NamedIndividual>
    


    <!-- http://purl.obolibrary.org/obo/GAZ_00140387 -->

    <owl:NamedIndividual rdf:about="http://purl.obolibrary.org/obo/GAZ_00140387">
        <obo:RO_0001025 rdf:resource="http://purl.obolibrary.org/obo/GAZ_00014088"/>
        <obo:IAO_0000115>Mountains, 15 mi long and 3 mi wide, rising to 2,100 m and extending S from Palestrina Glacier in the NW part of Alexander Island.</obo:IAO_0000115>
        <oboInOwl:hasOBONamespace>GAZ</oboInOwl:hasOBONamespace>
        <oboInOwl:id>GAZ:00140387</oboInOwl:id>
        <rdfs:label>Lassus Mountains</rdfs:label>
    </owl:NamedIndividual>
    


    <!-- http://purl.obolibrary.org/obo/GAZ_00140388 -->

    <owl:NamedIndividual rdf:about="http://purl.obolibrary.org/obo/GAZ_00140388">
        <obo:RO_0001025 rdf:resource="http://purl.obolibrary.org/obo/GAZ_00014088"/>
        <obo:IAO_0000115>A glacier in the N part of Alexander Island, 11 mi long and 8 mi wide, flowing W from Nichols Snowfield into Lazarev Bay.</obo:IAO_0000115>
        <oboInOwl:hasOBONamespace>GAZ</oboInOwl:hasOBONamespace>
        <oboInOwl:id>GAZ:00140388</oboInOwl:id>
        <rdfs:label>Palestrina Glacier</rdfs:label>
    </owl:NamedIndividual>
    


    <!-- http://purl.obolibrary.org/obo/GAZ_00140389 -->

    <owl:NamedIndividual rdf:about="http://purl.obolibrary.org/obo/GAZ_00140389">
        <obo:RO_0001025 rdf:resource="http://purl.obolibrary.org/obo/GAZ_00014088"/>
        <obo:IAO_0000115>A glacier flowing N into Palestrina Glacier, NW Alexander Island.</obo:IAO_0000115>
        <oboInOwl:hasOBONamespace>GAZ</oboInOwl:hasOBONamespace>
        <oboInOwl:id>GAZ:00140389</oboInOwl:id>
        <rdfs:label>McManus Glacier</rdfs:label>
    </owl:NamedIndividual>
    


    <!-- http://purl.obolibrary.org/obo/GAZ_00140390 -->

    <owl:NamedIndividual rdf:about="http://purl.obolibrary.org/obo/GAZ_00140390">
        <obo:RO_0001025 rdf:resource="http://purl.obolibrary.org/obo/GAZ_00140386"/>
        <obo:IAO_0000115>A nunatak which is reverse S-shaped, rising to c. 750 m just W of Tufts Pass in Nichols Snowfield, Alexander Island.</obo:IAO_0000115>
        <oboInOwl:hasOBONamespace>GAZ</oboInOwl:hasOBONamespace>
        <oboInOwl:id>GAZ:00140390</oboInOwl:id>
        <rdfs:label>Serpent Nunatak</rdfs:label>
    </owl:NamedIndividual>
    


    <!-- http://purl.obolibrary.org/obo/GAZ_00140391 -->

    <owl:NamedIndividual rdf:about="http://purl.obolibrary.org/obo/GAZ_00140391">
        <obo:RO_0001025 rdf:resource="http://purl.obolibrary.org/obo/GAZ_00140386"/>
        <obo:IAO_0000115>A nunatak rising to c. 800 m in Nichols Snowfield, N Alexander Island.</obo:IAO_0000115>
        <oboInOwl:hasOBONamespace>GAZ</oboInOwl:hasOBONamespace>
        <oboInOwl:id>GAZ:00140391</oboInOwl:id>
        <rdfs:label>Lizard Nunatak</rdfs:label>
    </owl:NamedIndividual>
    


    <!-- http://purl.obolibrary.org/obo/GAZ_00140392 -->

    <owl:NamedIndividual rdf:about="http://purl.obolibrary.org/obo/GAZ_00140392">
        <obo:RO_0001025 rdf:resource="http://purl.obolibrary.org/obo/GAZ_00014084"/>
        <obo:IAO_0000115>A rectangular bay, 28 km long and 24 km wide, between Alexander Island and Rothschild Island and bounded on the south by ice shelf joining the two islands.</obo:IAO_0000115>
        <oboInOwl:hasOBONamespace>GAZ</oboInOwl:hasOBONamespace>
        <oboInOwl:id>GAZ:00140392</oboInOwl:id>
        <rdfs:label>Lazarev Bay</rdfs:label>
    </owl:NamedIndividual>
    


    <!-- http://purl.obolibrary.org/obo/GAZ_00140398 -->

    <owl:NamedIndividual rdf:about="http://purl.obolibrary.org/obo/GAZ_00140398">
        <obo:RO_0001025 rdf:resource="http://purl.obolibrary.org/obo/GAZ_00140399"/>
        <obo:IAO_0000115>A small glacier in the northeast part of Noville Peninsula, Thurston Island. It flows northeast to Bellingshausen Sea between Mounts Palmer and Feury.</obo:IAO_0000115>
        <oboInOwl:hasOBONamespace>GAZ</oboInOwl:hasOBONamespace>
        <oboInOwl:id>GAZ:00140398</oboInOwl:id>
        <rdfs:label>Sikorski Glacier</rdfs:label>
    </owl:NamedIndividual>
    


    <!-- http://purl.obolibrary.org/obo/GAZ_00140399 -->

    <owl:NamedIndividual rdf:about="http://purl.obolibrary.org/obo/GAZ_00140399">
        <obo:RO_0001025 rdf:resource="http://purl.obolibrary.org/obo/GAZ_00014140"/>
        <obo:IAO_0000115>A high ice-covered peninsula about 30 mi long, between Peale and Murphy Inlets on the N side of Thurston Island.</obo:IAO_0000115>
        <oboInOwl:hasOBONamespace>GAZ</oboInOwl:hasOBONamespace>
        <oboInOwl:id>GAZ:00140399</oboInOwl:id>
        <rdfs:label>Noville Peninsula</rdfs:label>
    </owl:NamedIndividual>
    


    <!-- http://purl.obolibrary.org/obo/GAZ_00140462 -->

    <owl:NamedIndividual rdf:about="http://purl.obolibrary.org/obo/GAZ_00140462">
        <obo:RO_0001025 rdf:resource="http://purl.obolibrary.org/obo/GAZ_00023304"/>
        <obo:IAO_0000115>A small floating glacier tongue nourished by Simpson Glacier and Fendley Glacier as it extends into the sea between Nelson Cliff and Atkinson Cliffs, along the north coast of Victoria Land.</obo:IAO_0000115>
        <oboInOwl:hasOBONamespace>GAZ</oboInOwl:hasOBONamespace>
        <oboInOwl:id>GAZ:00140462</oboInOwl:id>
        <rdfs:label>Simpson Glacier Tongue</rdfs:label>
    </owl:NamedIndividual>
    


    <!-- http://purl.obolibrary.org/obo/GAZ_00140466 -->

    <owl:NamedIndividual rdf:about="http://purl.obolibrary.org/obo/GAZ_00140466">
        <obo:RO_0001025 rdf:resource="http://purl.obolibrary.org/obo/GAZ_00140467"/>
        <obo:IAO_0000115>An ice-covered island at the southwest extremity of Riiser-Larsen Ice Shelf, separating it from Brunt Ice Shelf, about 20 miles off the Princess Martha Coast. The island is about 45 miles long and has three narrow arms in the form of a trefoil.</obo:IAO_0000115>
        <oboInOwl:hasOBONamespace>GAZ</oboInOwl:hasOBONamespace>
        <oboInOwl:id>GAZ:00140466</oboInOwl:id>
        <rdfs:label>Lyddan Island</rdfs:label>
    </owl:NamedIndividual>
    


    <!-- http://purl.obolibrary.org/obo/GAZ_00140467 -->

    <owl:NamedIndividual rdf:about="http://purl.obolibrary.org/obo/GAZ_00140467">
        <obo:RO_0001025 rdf:resource="http://purl.obolibrary.org/obo/GAZ_00004045"/>
        <obo:IAO_0000115>An ice shelf about 400 km long on the coast of Queen Maud Land, extending from Cape Norvegia in the north to Lyddan Island and Stancomb-Wills Glacier in the south.</obo:IAO_0000115>
        <oboInOwl:hasOBONamespace>GAZ</oboInOwl:hasOBONamespace>
        <oboInOwl:id>GAZ:00140467</oboInOwl:id>
        <rdfs:label>Riiser-Larsen Ice Shelf</rdfs:label>
    </owl:NamedIndividual>
    


    <!-- http://purl.obolibrary.org/obo/GAZ_00140481 -->

    <owl:NamedIndividual rdf:about="http://purl.obolibrary.org/obo/GAZ_00140481">
        <obo:RO_0001025 rdf:resource="http://purl.obolibrary.org/obo/GAZ_00140102"/>
        <obo:IAO_0000115>An ice tongue that occupies the north half of Tripp Bay on the coast of Victoria Land. The feature is nurtured by several glaciers (Fry Glacier, Hedblom Glacier, as well as ice from Oates Piedmont Glacier).</obo:IAO_0000115>
        <oboInOwl:hasOBONamespace>GAZ</oboInOwl:hasOBONamespace>
        <oboInOwl:id>GAZ:00140481</oboInOwl:id>
        <rdfs:label>Tripp Ice Tongue</rdfs:label>
    </owl:NamedIndividual>
    


    <!-- http://purl.obolibrary.org/obo/GAZ_00140487 -->

    <owl:NamedIndividual rdf:about="http://purl.obolibrary.org/obo/GAZ_00140487">
        <obo:RO_0001025 rdf:resource="http://purl.obolibrary.org/obo/GAZ_00014088"/>
        <obo:IAO_0000115>A glacier on the east coast of Alexander Island, 32 km long and 10 km wide at its mouth, flowing east into George VI Sound immediately south of Fossil Bluff.</obo:IAO_0000115>
        <oboInOwl:hasOBONamespace>GAZ</oboInOwl:hasOBONamespace>
        <oboInOwl:id>GAZ:00140487</oboInOwl:id>
        <rdfs:label>Uranus Glacier</rdfs:label>
    </owl:NamedIndividual>
    


    <!-- http://purl.obolibrary.org/obo/GAZ_00140488 -->

    <owl:NamedIndividual rdf:about="http://purl.obolibrary.org/obo/GAZ_00140488">
        <obo:RO_0001025 rdf:resource="http://purl.obolibrary.org/obo/GAZ_00014088"/>
        <obo:IAO_0000115>A glacier encircled by Mariner Hill, Syrtis Hill, Natal Ridge, and Ares Cliff.</obo:IAO_0000115>
        <oboInOwl:hasOBONamespace>GAZ</oboInOwl:hasOBONamespace>
        <oboInOwl:id>GAZ:00140488</oboInOwl:id>
        <rdfs:label>Utopia Glacier</rdfs:label>
    </owl:NamedIndividual>
    


    <!-- http://purl.obolibrary.org/obo/GAZ_00140497 -->

    <owl:NamedIndividual rdf:about="http://purl.obolibrary.org/obo/GAZ_00140497">
        <obo:RO_0001025 rdf:resource="http://purl.obolibrary.org/obo/GAZ_00139422"/>
        <obo:IAO_0000115>A bay 6 km wide, indenting the coast immediately east of Utstikkar Glacier.</obo:IAO_0000115>
        <oboInOwl:hasOBONamespace>GAZ</oboInOwl:hasOBONamespace>
        <oboInOwl:id>GAZ:00140497</oboInOwl:id>
        <rdfs:label>Utstikkar Bay</rdfs:label>
    </owl:NamedIndividual>
    


    <!-- http://purl.obolibrary.org/obo/GAZ_00140504 -->

    <owl:NamedIndividual rdf:about="http://purl.obolibrary.org/obo/GAZ_00140504">
        <obo:RO_0001025 rdf:resource="http://purl.obolibrary.org/obo/GAZ_00014084"/>
        <obo:IAO_0000115>An ice shelf, 60 km long and 24 km wide, between Fletcher and Allison Peninsulas, Ellsworth Land.</obo:IAO_0000115>
        <oboInOwl:hasOBONamespace>GAZ</oboInOwl:hasOBONamespace>
        <oboInOwl:id>GAZ:00140504</oboInOwl:id>
        <rdfs:label>Venable Ice Shelf</rdfs:label>
    </owl:NamedIndividual>
    


    <!-- http://purl.obolibrary.org/obo/GAZ_00140505 -->

    <owl:NamedIndividual rdf:about="http://purl.obolibrary.org/obo/GAZ_00140505">
        <obo:RO_0001025 rdf:resource="http://purl.obolibrary.org/obo/GAZ_00140504"/>
        <obo:IAO_0000115>An ice stream about 24 km long flowing into Venable Ice Shelf just east of Fletcher Peninsula.</obo:IAO_0000115>
        <oboInOwl:hasOBONamespace>GAZ</oboInOwl:hasOBONamespace>
        <oboInOwl:id>GAZ:00140505</oboInOwl:id>
        <rdfs:label>Williams Ice Stream</rdfs:label>
    </owl:NamedIndividual>
    


    <!-- http://purl.obolibrary.org/obo/GAZ_00140506 -->

    <owl:NamedIndividual rdf:about="http://purl.obolibrary.org/obo/GAZ_00140506">
        <obo:RO_0001025 rdf:resource="http://purl.obolibrary.org/obo/GAZ_00017735"/>
        <obo:IAO_0000115>A glacier located on Greenwich Island, Antarctica and is bounded by Oborishte Ridge to the NW, Terter Peak and Razgrad Peak to the NE, and Ephraim Bluff to the SE.</obo:IAO_0000115>
        <oboInOwl:hasOBONamespace>GAZ</oboInOwl:hasOBONamespace>
        <oboInOwl:id>GAZ:00140506</oboInOwl:id>
        <rdfs:label>Wulfila Glacier</rdfs:label>
    </owl:NamedIndividual>
    


    <!-- http://purl.obolibrary.org/obo/GAZ_00140546 -->

    <owl:NamedIndividual rdf:about="http://purl.obolibrary.org/obo/GAZ_00140546">
        <obo:RO_0001025 rdf:resource="http://purl.obolibrary.org/obo/GAZ_00014140"/>
        <obo:IAO_0000115>A glacier in east Thurston Island; it flows east-northeast into Morgan Inlet between Tierney Peninsula and the promontory ending in Ryan Point.</obo:IAO_0000115>
        <oboInOwl:hasOBONamespace>GAZ</oboInOwl:hasOBONamespace>
        <oboInOwl:id>GAZ:00140546</oboInOwl:id>
        <rdfs:label>Zinberg Glacier</rdfs:label>
    </owl:NamedIndividual>
    


    <!-- http://purl.obolibrary.org/obo/GAZ_00140560 -->

    <owl:NamedIndividual rdf:about="http://purl.obolibrary.org/obo/GAZ_00140560">
        <obo:RO_0001025 rdf:resource="http://purl.obolibrary.org/obo/GAZ_00139119"/>
        <obo:IAO_0000115>A pro-glacial tidal lake in Ablation Valley, Alexander Island, with stratified saline and fresh water and depths exceeding 117 m. The feature is dammed in the upper portion by ice that pushes into the lake from the adjacent George VI Ice Shelf.</obo:IAO_0000115>
        <oboInOwl:hasOBONamespace>GAZ</oboInOwl:hasOBONamespace>
        <oboInOwl:id>GAZ:00140560</oboInOwl:id>
        <rdfs:label>Ablation Lake</rdfs:label>
    </owl:NamedIndividual>
    


    <!-- http://purl.obolibrary.org/obo/GAZ_00140631 -->

    <owl:NamedIndividual rdf:about="http://purl.obolibrary.org/obo/GAZ_00140631">
        <obo:RO_0001025 rdf:resource="http://purl.obolibrary.org/obo/GAZ_00009523"/>
        <obo:IAO_0000115>A rock 3.7 km southwest of Despair Rocks and 13 km northwest of Route Point, off the west end of Coronation Island in the South Orkney Islands.</obo:IAO_0000115>
        <oboInOwl:hasOBONamespace>GAZ</oboInOwl:hasOBONamespace>
        <oboInOwl:id>GAZ:00140631</oboInOwl:id>
        <rdfs:label>Lay-brother Rock</rdfs:label>
    </owl:NamedIndividual>
    


    <!-- http://purl.obolibrary.org/obo/GAZ_00140632 -->

    <owl:NamedIndividual rdf:about="http://purl.obolibrary.org/obo/GAZ_00140632">
        <obo:RO_0001025 rdf:resource="http://purl.obolibrary.org/obo/GAZ_00009523"/>
        <obo:IAO_0000115>A group of rocks 2 mi S of Melsom Rocks and 7.5 mi WSW of Penguin Point, the NW tip of Coronation Island, in the South Orkney Islands.</obo:IAO_0000115>
        <oboInOwl:hasOBONamespace>GAZ</oboInOwl:hasOBONamespace>
        <oboInOwl:id>GAZ:00140632</oboInOwl:id>
        <rdfs:label>Despair Rocks</rdfs:label>
    </owl:NamedIndividual>
    


    <!-- http://purl.obolibrary.org/obo/GAZ_00140633 -->

    <owl:NamedIndividual rdf:about="http://purl.obolibrary.org/obo/GAZ_00140633">
        <obo:RO_0001025 rdf:resource="http://purl.obolibrary.org/obo/GAZ_00009523"/>
        <obo:IAO_0000115>A group of isolated rocks lying 2 mi N of Despair Rocks and 7 mi W of Penguin Point, the NW end of Coronation Island, in the South Orkney Islands.</obo:IAO_0000115>
        <oboInOwl:hasOBONamespace>GAZ</oboInOwl:hasOBONamespace>
        <oboInOwl:id>GAZ:00140633</oboInOwl:id>
        <rdfs:label>Melsom Rocks</rdfs:label>
    </owl:NamedIndividual>
    


    <!-- http://purl.obolibrary.org/obo/GAZ_00140634 -->

    <owl:NamedIndividual rdf:about="http://purl.obolibrary.org/obo/GAZ_00140634">
        <obo:RO_0001025 rdf:resource="http://purl.obolibrary.org/obo/GAZ_00007328"/>
        <obo:IAO_0000115>An Antarctic island extending 700 m in south-north direction off the north coast of Greenwich Island in the South Shetland Islands.</obo:IAO_0000115>
        <oboInOwl:hasOBONamespace>GAZ</oboInOwl:hasOBONamespace>
        <oboInOwl:id>GAZ:00140634</oboInOwl:id>
        <rdfs:label>Kabile Island</rdfs:label>
    </owl:NamedIndividual>
    


    <!-- http://purl.obolibrary.org/obo/GAZ_00140635 -->

    <owl:NamedIndividual rdf:about="http://purl.obolibrary.org/obo/GAZ_00140635">
        <obo:RO_0001025 rdf:resource="http://purl.obolibrary.org/obo/GAZ_00007328"/>
        <obo:IAO_0000115>A narrow island which is marked by a series of small elevations throughout its length, lying 0.8 km northwest of Dee Island in the South Shetland Islands.</obo:IAO_0000115>
        <oboInOwl:hasOBONamespace>GAZ</oboInOwl:hasOBONamespace>
        <oboInOwl:id>GAZ:00140635</oboInOwl:id>
        <rdfs:label>Sierra Island</rdfs:label>
    </owl:NamedIndividual>
    


    <!-- http://purl.obolibrary.org/obo/GAZ_00140636 -->

    <owl:NamedIndividual rdf:about="http://purl.obolibrary.org/obo/GAZ_00140636">
        <obo:RO_0001025 rdf:resource="http://purl.obolibrary.org/obo/GAZ_00007328"/>
        <obo:IAO_0000115>An island with a conspicuous sharp peak at its S end, lying 2.5 mi E of Ongley Island, close off the N side of Greenwich Island in the South Shetland Islands.</obo:IAO_0000115>
        <oboInOwl:hasOBONamespace>GAZ</oboInOwl:hasOBONamespace>
        <oboInOwl:id>GAZ:00140636</oboInOwl:id>
        <rdfs:label>Dee Island</rdfs:label>
    </owl:NamedIndividual>
    


    <!-- http://purl.obolibrary.org/obo/GAZ_00140637 -->

    <owl:NamedIndividual rdf:about="http://purl.obolibrary.org/obo/GAZ_00140637">
        <obo:RO_0001025 rdf:resource="http://purl.obolibrary.org/obo/GAZ_00007328"/>
        <obo:IAO_0000115>A small island lying 2.5 mi W of Dee Island, close off the N side of Greenwich Island, in the South Shetland Islands.</obo:IAO_0000115>
        <oboInOwl:hasOBONamespace>GAZ</oboInOwl:hasOBONamespace>
        <oboInOwl:id>GAZ:00140637</oboInOwl:id>
        <rdfs:label>Ongley Island</rdfs:label>
    </owl:NamedIndividual>
    


    <!-- http://purl.obolibrary.org/obo/GAZ_00140638 -->

    <owl:NamedIndividual rdf:about="http://purl.obolibrary.org/obo/GAZ_00140638">
        <obo:RO_0001025 rdf:resource="http://purl.obolibrary.org/obo/GAZ_00140641"/>
        <obo:IAO_0000115>A 4 km long glacier on Smith Island, South Shetland Islands draining the northwest slopes of Imeon Range. Flowing southwest of Drinov Peak and west of Varshets Saddle southwestward along the northwest slopes of Antim Peak into Drake Passage south of Villagra Point.</obo:IAO_0000115>
        <oboInOwl:hasOBONamespace>GAZ</oboInOwl:hasOBONamespace>
        <oboInOwl:id>GAZ:00140638</oboInOwl:id>
        <rdfs:label>Chuprene Glacier</rdfs:label>
    </owl:NamedIndividual>
    


    <!-- http://purl.obolibrary.org/obo/GAZ_00140639 -->

    <owl:NamedIndividual rdf:about="http://purl.obolibrary.org/obo/GAZ_00140639">
        <rdf:type rdf:resource="http://purl.obolibrary.org/obo/ENVO_00000305"/>
        <obo:RO_0001025 rdf:resource="http://purl.obolibrary.org/obo/GAZ_00017745"/>
        <obo:IAO_0000115>A cape forming the north end of Smith Island, in the South Shetland Islands.</obo:IAO_0000115>
        <oboInOwl:hasOBONamespace>GAZ</oboInOwl:hasOBONamespace>
        <oboInOwl:id>GAZ:00140639</oboInOwl:id>
        <rdfs:label>Cape Smith</rdfs:label>
    </owl:NamedIndividual>
    


    <!-- http://purl.obolibrary.org/obo/GAZ_00140640 -->

    <owl:NamedIndividual rdf:about="http://purl.obolibrary.org/obo/GAZ_00140640">
        <obo:RO_0001025 rdf:resource="http://purl.obolibrary.org/obo/GAZ_00140641"/>
        <obo:IAO_0000115>A 3 km long glacier on Smith Island, South Shetland Islands draining the southeast slopes of Imeon Range southeast of Slaveykov Peak and east of Neofit Peak. Flowing southeastward into Bransfield Strait southwest of Ivan Asen Point.</obo:IAO_0000115>
        <oboInOwl:hasOBONamespace>GAZ</oboInOwl:hasOBONamespace>
        <oboInOwl:id>GAZ:00140640</oboInOwl:id>
        <rdfs:label>Armira Glacier</rdfs:label>
    </owl:NamedIndividual>
    


    <!-- http://purl.obolibrary.org/obo/GAZ_00140641 -->

    <owl:NamedIndividual rdf:about="http://purl.obolibrary.org/obo/GAZ_00140641">
        <obo:RO_0001025 rdf:resource="http://purl.obolibrary.org/obo/GAZ_00017745"/>
        <obo:IAO_0000115>A mountain range occupying the interior of Smith Island in the South Shetland Islands, Antarctica. Extending 30 km in southwest-northeast direction between Cape James and Cape Smith, and 6.8 km wide.</obo:IAO_0000115>
        <oboInOwl:hasOBONamespace>GAZ</oboInOwl:hasOBONamespace>
        <oboInOwl:id>GAZ:00140641</oboInOwl:id>
        <rdfs:label>Imeon Range</rdfs:label>
    </owl:NamedIndividual>
    


    <!-- http://purl.obolibrary.org/obo/GAZ_00140642 -->

    <owl:NamedIndividual rdf:about="http://purl.obolibrary.org/obo/GAZ_00140642">
        <rdf:type rdf:resource="http://purl.obolibrary.org/obo/ENVO_00000305"/>
        <obo:RO_0001025 rdf:resource="http://purl.obolibrary.org/obo/GAZ_00017745"/>
        <obo:IAO_0000115>A headland on the northwest coast of Smith Island, South Shetland Islands situated 3.9 km west-southwest of Cape Smith, 9.9 km northeast of Gregory Point, and 3.5 km North-northeast of Mount Christi.</obo:IAO_0000115>
        <oboInOwl:hasOBONamespace>GAZ</oboInOwl:hasOBONamespace>
        <oboInOwl:id>GAZ:00140642</oboInOwl:id>
        <rdfs:label>Delyan Point</rdfs:label>
    </owl:NamedIndividual>
    


    <!-- http://purl.obolibrary.org/obo/GAZ_00140643 -->

    <owl:NamedIndividual rdf:about="http://purl.obolibrary.org/obo/GAZ_00140643">
        <obo:RO_0001025 rdf:resource="http://purl.obolibrary.org/obo/GAZ_00140641"/>
        <obo:IAO_0000115>A 2.6 km long glacier on Smith Island, South Shetland Islands draining the southeast slopes of Imeon Range southeast of Zavet Saddle and south of the summit Mount Foster. Flowing southeastward into Ivan Asen Cove.</obo:IAO_0000115>
        <oboInOwl:hasOBONamespace>GAZ</oboInOwl:hasOBONamespace>
        <oboInOwl:id>GAZ:00140643</oboInOwl:id>
        <rdfs:label>Dragoman Glacier</rdfs:label>
    </owl:NamedIndividual>
    


    <!-- http://purl.obolibrary.org/obo/GAZ_00140644 -->

    <owl:NamedIndividual rdf:about="http://purl.obolibrary.org/obo/GAZ_00140644">
        <rdf:type rdf:resource="http://purl.obolibrary.org/obo/ENVO_00000305"/>
        <obo:RO_0001025 rdf:resource="http://purl.obolibrary.org/obo/GAZ_00017745"/>
        <obo:IAO_0000115>A cape which forms the south tip of Smith Island, in the South Shetland Islands.</obo:IAO_0000115>
        <oboInOwl:hasOBONamespace>GAZ</oboInOwl:hasOBONamespace>
        <oboInOwl:id>GAZ:00140644</oboInOwl:id>
        <rdfs:label>Cape James</rdfs:label>
    </owl:NamedIndividual>
    


    <!-- http://purl.obolibrary.org/obo/GAZ_00140645 -->

    <owl:NamedIndividual rdf:about="http://purl.obolibrary.org/obo/GAZ_00140645">
        <rdf:type rdf:resource="http://purl.obolibrary.org/obo/ENVO_00000305"/>
        <obo:RO_0001025 rdf:resource="http://purl.obolibrary.org/obo/GAZ_00017745"/>
        <obo:IAO_0000115>A headland forming the northeast side of the entrance to Hisarya Cove in Smith Island, South Shetland Islands. Situated 8.4 km northeast of Cape James.</obo:IAO_0000115>
        <oboInOwl:hasOBONamespace>GAZ</oboInOwl:hasOBONamespace>
        <oboInOwl:id>GAZ:00140645</oboInOwl:id>
        <rdfs:label>Dupnitsa Point</rdfs:label>
    </owl:NamedIndividual>
    


    <!-- http://purl.obolibrary.org/obo/GAZ_00140646 -->

    <owl:NamedIndividual rdf:about="http://purl.obolibrary.org/obo/GAZ_00140646">
        <rdf:type rdf:resource="http://purl.obolibrary.org/obo/ENVO_00000305"/>
        <obo:RO_0001025 rdf:resource="http://purl.obolibrary.org/obo/GAZ_00017745"/>
        <obo:IAO_0000115>A headland on the northwest coast of Smith Island, South Shetland Islands situated 7 km north-northeast of Cape James.</obo:IAO_0000115>
        <oboInOwl:hasOBONamespace>GAZ</oboInOwl:hasOBONamespace>
        <oboInOwl:id>GAZ:00140646</oboInOwl:id>
        <rdfs:label>Batak Point</rdfs:label>
    </owl:NamedIndividual>
    


    <!-- http://purl.obolibrary.org/obo/GAZ_00140647 -->

    <owl:NamedIndividual rdf:about="http://purl.obolibrary.org/obo/GAZ_00140647">
        <rdf:type rdf:resource="http://purl.obolibrary.org/obo/ENVO_00000305"/>
        <obo:RO_0001025 rdf:resource="http://purl.obolibrary.org/obo/GAZ_00017745"/>
        <obo:IAO_0000115>A headland on the northwest coast of Smith Island, South Shetland Islands situated 13 km north-northeast of Cape James and 18.3 km southwest of Cape Smith.</obo:IAO_0000115>
        <oboInOwl:hasOBONamespace>GAZ</oboInOwl:hasOBONamespace>
        <oboInOwl:id>GAZ:00140647</oboInOwl:id>
        <rdfs:label>Garmen Point</rdfs:label>
    </owl:NamedIndividual>
    


    <!-- http://purl.obolibrary.org/obo/GAZ_00140648 -->

    <owl:NamedIndividual rdf:about="http://purl.obolibrary.org/obo/GAZ_00140648">
        <obo:RO_0001025 rdf:resource="http://purl.obolibrary.org/obo/GAZ_00140641"/>
        <obo:IAO_0000115>A 3.4 km long glacier on Smith Island, South Shetland Islands draining the northwest slopes of Imeon Range. Flowing north of Mount Pisgah and northwest of Mezek Peak into Drake Passage.</obo:IAO_0000115>
        <oboInOwl:hasOBONamespace>GAZ</oboInOwl:hasOBONamespace>
        <oboInOwl:id>GAZ:00140648</oboInOwl:id>
        <rdfs:label>Dalgopol Glacier</rdfs:label>
    </owl:NamedIndividual>
    


    <!-- http://purl.obolibrary.org/obo/GAZ_00140649 -->

    <owl:NamedIndividual rdf:about="http://purl.obolibrary.org/obo/GAZ_00140649">
        <obo:RO_0001025 rdf:resource="http://purl.obolibrary.org/obo/GAZ_00140059"/>
        <obo:IAO_0000115>A cove on the southeast coast of Smith Island in the South Shetland Islands, Antarctica, to the N of Ivan Asen Point.</obo:IAO_0000115>
        <oboInOwl:hasOBONamespace>GAZ</oboInOwl:hasOBONamespace>
        <oboInOwl:id>GAZ:00140649</oboInOwl:id>
        <rdfs:label>Ivan Asen Cove</rdfs:label>
    </owl:NamedIndividual>
    


    <!-- http://purl.obolibrary.org/obo/GAZ_00140650 -->

    <owl:NamedIndividual rdf:about="http://purl.obolibrary.org/obo/GAZ_00140650">
        <rdf:type rdf:resource="http://purl.obolibrary.org/obo/ENVO_00000305"/>
        <obo:RO_0001025 rdf:resource="http://purl.obolibrary.org/obo/GAZ_00017745"/>
        <obo:IAO_0000115>A headland on the northwest coast of Smith Island, South Shetland Islands situated 10.5 km north-northeast of Cape James and 20.5 km southwest of Cape Smith. Formed by an offshoot of Neofit Peak.</obo:IAO_0000115>
        <oboInOwl:hasOBONamespace>GAZ</oboInOwl:hasOBONamespace>
        <oboInOwl:id>GAZ:00140650</oboInOwl:id>
        <rdfs:label>Lakatnik Point</rdfs:label>
    </owl:NamedIndividual>
    


    <!-- http://purl.obolibrary.org/obo/GAZ_00140651 -->

    <owl:NamedIndividual rdf:about="http://purl.obolibrary.org/obo/GAZ_00140651">
        <rdf:type rdf:resource="http://purl.obolibrary.org/obo/ENVO_00000305"/>
        <obo:RO_0001025 rdf:resource="http://purl.obolibrary.org/obo/GAZ_00017745"/>
        <obo:IAO_0000115>A headland on the northwest coast of Smith Island, South Shetland Islands situated 4.5 km north-northeast of Cape James.</obo:IAO_0000115>
        <oboInOwl:hasOBONamespace>GAZ</oboInOwl:hasOBONamespace>
        <oboInOwl:id>GAZ:00140651</oboInOwl:id>
        <rdfs:label>Elin Pelin Point</rdfs:label>
    </owl:NamedIndividual>
    


    <!-- http://purl.obolibrary.org/obo/GAZ_00140652 -->

    <owl:NamedIndividual rdf:about="http://purl.obolibrary.org/obo/GAZ_00140652">
        <obo:RO_0001025 rdf:resource="http://purl.obolibrary.org/obo/GAZ_00017745"/>
        <obo:IAO_0000115>A narrow rocky point projecting 300 m from the southeast coast of Smith Island in the South Shetland Islands, Antarctica. Situated 12 km northeast of Cape James, 20.6 km southwest of Cape Smith, 3.7 km south-southeast of the island&apos;s summit Mount Foster (2105 m), and 3.2 km southeast of Slaveykov Peak. Forming the south side of the entrance to an 1.2 km wide cove indenting the coast for 400 m, and named Ivan Asen Cove in association with the point.</obo:IAO_0000115>
        <oboInOwl:hasOBONamespace>GAZ</oboInOwl:hasOBONamespace>
        <oboInOwl:id>GAZ:00140652</oboInOwl:id>
        <rdfs:label>Ivan Asen Point</rdfs:label>
    </owl:NamedIndividual>
    


    <!-- http://purl.obolibrary.org/obo/GAZ_00140653 -->

    <owl:NamedIndividual rdf:about="http://purl.obolibrary.org/obo/GAZ_00140653">
        <rdf:type rdf:resource="http://purl.obolibrary.org/obo/ENVO_00000305"/>
        <obo:RO_0001025 rdf:resource="http://purl.obolibrary.org/obo/GAZ_00017745"/>
        <obo:IAO_0000115>A headland on the southeast coast of Smith Island, South Shetland Islands situated 3.6 km east-northeast of Cape James.</obo:IAO_0000115>
        <oboInOwl:hasOBONamespace>GAZ</oboInOwl:hasOBONamespace>
        <oboInOwl:id>GAZ:00140653</oboInOwl:id>
        <rdfs:label>Suhindol Point</rdfs:label>
    </owl:NamedIndividual>
    


    <!-- http://purl.obolibrary.org/obo/GAZ_00140654 -->

    <owl:NamedIndividual rdf:about="http://purl.obolibrary.org/obo/GAZ_00140654">
        <rdf:type rdf:resource="http://purl.obolibrary.org/obo/ENVO_00000305"/>
        <obo:RO_0001025 rdf:resource="http://purl.obolibrary.org/obo/GAZ_00017745"/>
        <obo:IAO_0000115>A headland on the northwest coast of Smith Island, South Shetland Islands situated 12.8 km southwest of Cape Smith and 2 km north of Gregory Point.</obo:IAO_0000115>
        <oboInOwl:hasOBONamespace>GAZ</oboInOwl:hasOBONamespace>
        <oboInOwl:id>GAZ:00140654</oboInOwl:id>
        <rdfs:label>Markeli Point</rdfs:label>
    </owl:NamedIndividual>
    


    <!-- http://purl.obolibrary.org/obo/GAZ_00140655 -->

    <owl:NamedIndividual rdf:about="http://purl.obolibrary.org/obo/GAZ_00140655">
        <obo:RO_0001025 rdf:resource="http://purl.obolibrary.org/obo/GAZ_00140641"/>
        <obo:IAO_0000115>A 2.7 km long glacier on Smith Island, South Shetland Islands draining the northwest slopes of Imeon Range. Flowing west of Mount Christi into Drake Passage.</obo:IAO_0000115>
        <oboInOwl:hasOBONamespace>GAZ</oboInOwl:hasOBONamespace>
        <oboInOwl:id>GAZ:00140655</oboInOwl:id>
        <rdfs:label>Kongur Glacier</rdfs:label>
    </owl:NamedIndividual>
    


    <!-- http://purl.obolibrary.org/obo/GAZ_00140656 -->

    <owl:NamedIndividual rdf:about="http://purl.obolibrary.org/obo/GAZ_00140656">
        <obo:RO_0001025 rdf:resource="http://purl.obolibrary.org/obo/GAZ_00140641"/>
        <obo:IAO_0000115>A 3 km long glacier on Smith Island, South Shetland Islands draining the southeast slopes of Imeon Range east of Riggs Peak and south of Neofit Peak. Flowing southeastward into Bransfield Strait.</obo:IAO_0000115>
        <oboInOwl:hasOBONamespace>GAZ</oboInOwl:hasOBONamespace>
        <oboInOwl:id>GAZ:00140656</oboInOwl:id>
        <rdfs:label>Gramada Glacier</rdfs:label>
    </owl:NamedIndividual>
    


    <!-- http://purl.obolibrary.org/obo/GAZ_00140657 -->

    <owl:NamedIndividual rdf:about="http://purl.obolibrary.org/obo/GAZ_00140657">
        <obo:RO_0001025 rdf:resource="http://purl.obolibrary.org/obo/GAZ_00140641"/>
        <obo:IAO_0000115>A 3.8 km long glacier on Smith Island, South Shetland Islands draining the southeast slopes of Imeon Range east and southeast of Antim Peak, and south of Slatina Peak. Flowing southeastward into Bransfield Strait.</obo:IAO_0000115>
        <oboInOwl:hasOBONamespace>GAZ</oboInOwl:hasOBONamespace>
        <oboInOwl:id>GAZ:00140657</oboInOwl:id>
        <rdfs:label>Krivodol Glacier</rdfs:label>
    </owl:NamedIndividual>
    


    <!-- http://purl.obolibrary.org/obo/GAZ_00140658 -->

    <owl:NamedIndividual rdf:about="http://purl.obolibrary.org/obo/GAZ_00140658">
        <obo:RO_0001025 rdf:resource="http://purl.obolibrary.org/obo/GAZ_00140641"/>
        <obo:IAO_0000115>A 1.8 km long glacier on Smith Island, South Shetland Islands draining the southeast slopes of Imeon Range east of Organa Peak and south of Riggs Peak. Flowing southeastward into Hisarya Cove.</obo:IAO_0000115>
        <oboInOwl:hasOBONamespace>GAZ</oboInOwl:hasOBONamespace>
        <oboInOwl:id>GAZ:00140658</oboInOwl:id>
        <rdfs:label>Letnitsa Glacier</rdfs:label>
    </owl:NamedIndividual>
    


    <!-- http://purl.obolibrary.org/obo/GAZ_00140659 -->

    <owl:NamedIndividual rdf:about="http://purl.obolibrary.org/obo/GAZ_00140659">
        <obo:RO_0001025 rdf:resource="http://purl.obolibrary.org/obo/GAZ_00140641"/>
        <obo:IAO_0000115>A 3.5 km long glacier on Smith Island, South Shetland Islands draining the southeast slopes of Imeon Range east-southeast of Drinov Peak. Flowing east-southeastward into Bransfield Strait.</obo:IAO_0000115>
        <oboInOwl:hasOBONamespace>GAZ</oboInOwl:hasOBONamespace>
        <oboInOwl:id>GAZ:00140659</oboInOwl:id>
        <rdfs:label>Ovech Glacier</rdfs:label>
    </owl:NamedIndividual>
    


    <!-- http://purl.obolibrary.org/obo/GAZ_00140660 -->

    <owl:NamedIndividual rdf:about="http://purl.obolibrary.org/obo/GAZ_00140660">
        <obo:RO_0001025 rdf:resource="http://purl.obolibrary.org/obo/GAZ_00140059"/>
        <obo:IAO_0000115>A 950 m wide cove indenting for 500 m the southeast coast of Smith Island, South Shetland Islands 7.3 km northeast of Cape James.</obo:IAO_0000115>
        <oboInOwl:hasOBONamespace>GAZ</oboInOwl:hasOBONamespace>
        <oboInOwl:id>GAZ:00140660</oboInOwl:id>
        <rdfs:label>Hisarya Cove</rdfs:label>
    </owl:NamedIndividual>
    


    <!-- http://purl.obolibrary.org/obo/GAZ_00140661 -->

    <owl:NamedIndividual rdf:about="http://purl.obolibrary.org/obo/GAZ_00140661">
        <obo:RO_0001025 rdf:resource="http://purl.obolibrary.org/obo/GAZ_00140641"/>
        <obo:IAO_0000115>A 2.9 km long glacier on Smith Island, South Shetland Islands draining the southeast slopes of Imeon Range east of the summit Mount Foster and southeast of Evlogi Peak. Flowing southeastward into Bransfield Strait.</obo:IAO_0000115>
        <oboInOwl:hasOBONamespace>GAZ</oboInOwl:hasOBONamespace>
        <oboInOwl:id>GAZ:00140661</oboInOwl:id>
        <rdfs:label>Rupite Glacier</rdfs:label>
    </owl:NamedIndividual>
    


    <!-- http://purl.obolibrary.org/obo/GAZ_00140662 -->

    <owl:NamedIndividual rdf:about="http://purl.obolibrary.org/obo/GAZ_00140662">
        <obo:RO_0001025 rdf:resource="http://purl.obolibrary.org/obo/GAZ_00140641"/>
        <obo:IAO_0000115>A 1.8 km long glacier on Smith Island, South Shetland Islands draining the northwest slopes of Imeon Range. Flowing west of Drinov Peak into Cabut Cove.</obo:IAO_0000115>
        <oboInOwl:hasOBONamespace>GAZ</oboInOwl:hasOBONamespace>
        <oboInOwl:id>GAZ:00140662</oboInOwl:id>
        <rdfs:label>Yablanitsa Glacier</rdfs:label>
    </owl:NamedIndividual>
    


    <!-- http://purl.obolibrary.org/obo/GAZ_00140663 -->

    <owl:NamedIndividual rdf:about="http://purl.obolibrary.org/obo/GAZ_00140663">
        <obo:RO_0001025 rdf:resource="http://purl.obolibrary.org/obo/GAZ_00140641"/>
        <obo:IAO_0000115>A 3.2 km long glacier on Smith Island, South Shetland Islands draining the northwest slopes of Imeon Range. Flowing north of Drinov Peak into Drake Passage.</obo:IAO_0000115>
        <oboInOwl:hasOBONamespace>GAZ</oboInOwl:hasOBONamespace>
        <oboInOwl:id>GAZ:00140663</oboInOwl:id>
        <rdfs:label>Vetrino Glacier</rdfs:label>
    </owl:NamedIndividual>
    


    <!-- http://purl.obolibrary.org/obo/GAZ_00140664 -->

    <owl:NamedIndividual rdf:about="http://purl.obolibrary.org/obo/GAZ_00140664">
        <obo:RO_0001025 rdf:resource="http://purl.obolibrary.org/obo/GAZ_00140641"/>
        <obo:IAO_0000115>A 1.8 km long and 2 km wide glacier on Smith Island, South Shetland Islands draining the northwest slopes of Imeon Range. Flowing north of Mount Christi into Vedena Cove.</obo:IAO_0000115>
        <oboInOwl:hasOBONamespace>GAZ</oboInOwl:hasOBONamespace>
        <oboInOwl:id>GAZ:00140664</oboInOwl:id>
        <rdfs:label>Saparevo Glacier</rdfs:label>
    </owl:NamedIndividual>
    


    <!-- http://purl.obolibrary.org/obo/GAZ_00140665 -->

    <owl:NamedIndividual rdf:about="http://purl.obolibrary.org/obo/GAZ_00140665">
        <obo:RO_0001025 rdf:resource="http://purl.obolibrary.org/obo/GAZ_00140059"/>
        <obo:IAO_0000115>A 1.73 km wide cove indenting for 560 m the northwest coast of Smith Island, South Shetland Islands west of Delyan Point.</obo:IAO_0000115>
        <oboInOwl:hasOBONamespace>GAZ</oboInOwl:hasOBONamespace>
        <oboInOwl:id>GAZ:00140665</oboInOwl:id>
        <rdfs:label>Vedena Cove</rdfs:label>
    </owl:NamedIndividual>
    


    <!-- http://purl.obolibrary.org/obo/GAZ_00140666 -->

    <owl:NamedIndividual rdf:about="http://purl.obolibrary.org/obo/GAZ_00140666">
        <obo:RO_0001025 rdf:resource="http://purl.obolibrary.org/obo/GAZ_00139754"/>
        <obo:IAO_0000115>A roughly crescent-shaped snowfield draining the west slopes of Oryahovo Heights and the north slopes of Rotch Dome into Barclay Bay between Mercury Bluff and Rowe Point, Livingston Island. It extends 5 km inland, and 15 km in south-southwest to north-northeast direction.</obo:IAO_0000115>
        <oboInOwl:hasOBONamespace>GAZ</oboInOwl:hasOBONamespace>
        <oboInOwl:id>GAZ:00140666</oboInOwl:id>
        <rdfs:label>Etar Snowfield</rdfs:label>
    </owl:NamedIndividual>
    


    <!-- http://purl.obolibrary.org/obo/GAZ_00140667 -->

    <owl:NamedIndividual rdf:about="http://purl.obolibrary.org/obo/GAZ_00140667">
        <obo:RO_0001025 rdf:resource="http://purl.obolibrary.org/obo/GAZ_00140011"/>
        <obo:IAO_0000115>A rocky 410m peak in lower Huron Glacier, Livingston Island.</obo:IAO_0000115>
        <oboInOwl:hasOBONamespace>GAZ</oboInOwl:hasOBONamespace>
        <oboInOwl:id>GAZ:00140667</oboInOwl:id>
        <rdfs:label>Godech Nunatak</rdfs:label>
    </owl:NamedIndividual>
    


    <!-- http://purl.obolibrary.org/obo/GAZ_00140668 -->

    <owl:NamedIndividual rdf:about="http://purl.obolibrary.org/obo/GAZ_00140668">
        <obo:RO_0001025 rdf:resource="http://purl.obolibrary.org/obo/GAZ_00007329"/>
        <obo:IAO_0000115>A coast in eastern Livingston Island, extending 2.3 km from Hesperides Point to the southwest to Perunika Glacier to the northeast, forming the southeast coast of Emona Anchorage.</obo:IAO_0000115>
        <oboInOwl:hasOBONamespace>GAZ</oboInOwl:hasOBONamespace>
        <oboInOwl:id>GAZ:00140668</oboInOwl:id>
        <rdfs:label>Bulgarian Beach</rdfs:label>
    </owl:NamedIndividual>
    


    <!-- http://purl.obolibrary.org/obo/GAZ_00140669 -->

    <owl:NamedIndividual rdf:about="http://purl.obolibrary.org/obo/GAZ_00140669">
        <obo:RO_0001025 rdf:resource="http://purl.obolibrary.org/obo/GAZ_00140668"/>
        <obo:IAO_0000115>A 1 ha lagoon of elevation 2.4 m on Bulgarian Beach in eastern Livingston Island, in the South Shetland Islands. Formed by Rezovski Creek and separated from sea by a moraine of elevation near 3 m. Surmounted by the nameless hill rising to 36 m and located between Hesperides Hill and Sinemorets Hill.</obo:IAO_0000115>
        <oboInOwl:hasOBONamespace>GAZ</oboInOwl:hasOBONamespace>
        <oboInOwl:id>GAZ:00140669</oboInOwl:id>
        <rdfs:label>Grand Lagoon</rdfs:label>
    </owl:NamedIndividual>
    


    <!-- http://purl.obolibrary.org/obo/GAZ_00140670 -->

    <owl:NamedIndividual rdf:about="http://purl.obolibrary.org/obo/GAZ_00140670">
        <obo:RO_0001025 rdf:resource="http://purl.obolibrary.org/obo/GAZ_00007329"/>
        <obo:IAO_0000115>A melt-water stream located on Livingston Island, Antarctica. The 500 m long melt-water stream draining that portion of the northwestern slope of Balkan Snowfield located between Hesperides Hill, Atlantic Club Ridge, Krum Rock and Sinemorets Hill in eastern Livingston Island. Its lower course forms Grand Lagoon, and has its mouth at the SW extremity of Bulgarian Beach.</obo:IAO_0000115>
        <oboInOwl:hasOBONamespace>GAZ</oboInOwl:hasOBONamespace>
        <oboInOwl:id>GAZ:00140670</oboInOwl:id>
        <rdfs:label>Rezovski Creek</rdfs:label>
    </owl:NamedIndividual>
    


    <!-- http://purl.obolibrary.org/obo/GAZ_00140671 -->

    <owl:NamedIndividual rdf:about="http://purl.obolibrary.org/obo/GAZ_00140671">
        <obo:RO_0001025 rdf:resource="http://purl.obolibrary.org/obo/GAZ_00140059"/>
        <obo:IAO_0000115>A 2 km wide cove indenting for 1.2 km the S coast of Livingston Island (in the South Shetland Islands) that is entered between Elephant Point and Bond Point.</obo:IAO_0000115>
        <oboInOwl:hasOBONamespace>GAZ</oboInOwl:hasOBONamespace>
        <oboInOwl:id>GAZ:00140671</oboInOwl:id>
        <rdfs:label>Kavarna Cove</rdfs:label>
    </owl:NamedIndividual>
    


    <!-- http://purl.obolibrary.org/obo/GAZ_00140672 -->

    <owl:NamedIndividual rdf:about="http://purl.obolibrary.org/obo/GAZ_00140672">
        <obo:RO_0001025 rdf:resource="http://purl.obolibrary.org/obo/GAZ_00140020"/>
        <obo:IAO_0000115>A heavily crevassed depression in Perunika Glacier extending 2.7 km westwards from Rezen Knoll in eastern Livingston Island. The gully ends in the indentation forming the E corner of Emona Anchorage, and located 930 m SE by S of Aleko Rock and 3 km NE of Hesperides Point.</obo:IAO_0000115>
        <oboInOwl:hasOBONamespace>GAZ</oboInOwl:hasOBONamespace>
        <oboInOwl:id>GAZ:00140672</oboInOwl:id>
        <rdfs:label>Kresna Gully</rdfs:label>
    </owl:NamedIndividual>
    


    <!-- http://purl.obolibrary.org/obo/GAZ_00140673 -->

    <owl:NamedIndividual rdf:about="http://purl.obolibrary.org/obo/GAZ_00140673">
        <obo:RO_0001025 rdf:resource="http://purl.obolibrary.org/obo/GAZ_00140011"/>
        <obo:IAO_0000115>A pair of rocky peaks of elevation 320 m in middle Huron Glacier Livingston Island; 150 m away from each other.</obo:IAO_0000115>
        <oboInOwl:hasOBONamespace>GAZ</oboInOwl:hasOBONamespace>
        <oboInOwl:id>GAZ:00140673</oboInOwl:id>
        <rdfs:label>Kukeri Nunataks</rdfs:label>
    </owl:NamedIndividual>
    


    <!-- http://purl.obolibrary.org/obo/GAZ_00140674 -->

    <owl:NamedIndividual rdf:about="http://purl.obolibrary.org/obo/GAZ_00140674">
        <obo:RO_0001025 rdf:resource="http://purl.obolibrary.org/obo/GAZ_00140011"/>
        <obo:IAO_0000115>A 440m peak in upper Huron Glacier, Livingston Island.</obo:IAO_0000115>
        <oboInOwl:hasOBONamespace>GAZ</oboInOwl:hasOBONamespace>
        <oboInOwl:id>GAZ:00140674</oboInOwl:id>
        <rdfs:label>Lozen Nunatak</rdfs:label>
    </owl:NamedIndividual>
    


    <!-- http://purl.obolibrary.org/obo/GAZ_00140675 -->

    <owl:NamedIndividual rdf:about="http://purl.obolibrary.org/obo/GAZ_00140675">
        <obo:RO_0001025 rdf:resource="http://purl.obolibrary.org/obo/GAZ_00140011"/>
        <obo:IAO_0000115>A pair of rocky peaks of elevation 470m and 520m in middle Huron Glacier, Livingston Island, Antarctica; 250m away from each other.</obo:IAO_0000115>
        <oboInOwl:hasOBONamespace>GAZ</oboInOwl:hasOBONamespace>
        <oboInOwl:id>GAZ:00140675</oboInOwl:id>
        <rdfs:label>Nestinari Nunataks</rdfs:label>
    </owl:NamedIndividual>
    


    <!-- http://purl.obolibrary.org/obo/GAZ_00140676 -->

    <owl:NamedIndividual rdf:about="http://purl.obolibrary.org/obo/GAZ_00140676">
        <obo:RO_0001025 rdf:resource="http://purl.obolibrary.org/obo/GAZ_00007329"/>
        <obo:IAO_0000115>The portion of the northwest coast of South Bay, Livingston Island, Antarctica bounded to the southwest by Ereby Point and to the northeast by the north corner of the bay marked by an ice sea cave located 5.8 km east-northeast of Ereby Point and 1.45 km northwest of Aleko Point.</obo:IAO_0000115>
        <oboInOwl:hasOBONamespace>GAZ</oboInOwl:hasOBONamespace>
        <oboInOwl:id>GAZ:00140676</oboInOwl:id>
        <rdfs:label>Pimpirev Beach</rdfs:label>
    </owl:NamedIndividual>
    


    <!-- http://purl.obolibrary.org/obo/GAZ_00140677 -->

    <owl:NamedIndividual rdf:about="http://purl.obolibrary.org/obo/GAZ_00140677">
        <obo:RO_0001025 rdf:resource="http://purl.obolibrary.org/obo/GAZ_00139803"/>
        <obo:IAO_0000115>A rocky peak of elevation 430m in Vidin Heights, Livingston Island, Antarctica.</obo:IAO_0000115>
        <oboInOwl:hasOBONamespace>GAZ</oboInOwl:hasOBONamespace>
        <oboInOwl:id>GAZ:00140677</oboInOwl:id>
        <rdfs:label>Rakovski Nunatak</rdfs:label>
    </owl:NamedIndividual>
    


    <!-- http://purl.obolibrary.org/obo/GAZ_00140678 -->

    <owl:NamedIndividual rdf:about="http://purl.obolibrary.org/obo/GAZ_00140678">
        <obo:RO_0001025 rdf:resource="http://purl.obolibrary.org/obo/GAZ_00140022"/>
        <obo:IAO_0000115>A moraine reef in the Emona Anchorage in the eastern parts of Livingston Island, South Shetland Islands, Antarctica. The reef emerged during a recent glacier retreat.</obo:IAO_0000115>
        <oboInOwl:hasOBONamespace>GAZ</oboInOwl:hasOBONamespace>
        <oboInOwl:id>GAZ:00140678</oboInOwl:id>
        <rdfs:label>Rongel Reef</rdfs:label>
    </owl:NamedIndividual>
    


    <!-- http://purl.obolibrary.org/obo/GAZ_00140679 -->

    <owl:NamedIndividual rdf:about="http://purl.obolibrary.org/obo/GAZ_00140679">
        <obo:RO_0001025 rdf:resource="http://purl.obolibrary.org/obo/GAZ_00007329"/>
        <obo:IAO_0000115>A beach that faces False Bay on Livingston Island, Antarctica and extends for 4km on the Rozhen Peninsula between Charity Glacier and the Ruen Icefall. The beach is surmounted by Canetti Peak (400m) and MacKay Peak (approx 700m).</obo:IAO_0000115>
        <oboInOwl:hasOBONamespace>GAZ</oboInOwl:hasOBONamespace>
        <oboInOwl:id>GAZ:00140679</oboInOwl:id>
        <rdfs:label>Zagore Beach</rdfs:label>
    </owl:NamedIndividual>
    


    <!-- http://purl.obolibrary.org/obo/GAZ_00140680 -->

    <owl:NamedIndividual rdf:about="http://purl.obolibrary.org/obo/GAZ_00140680">
        <obo:RO_0001025 rdf:resource="http://purl.obolibrary.org/obo/GAZ_00140059"/>
        <obo:IAO_0000115>A group of rocks off Bulgarian Beach in eastern Livingston Island, Antarctica, consisting of one main rock, and two adjacent smaller ones submerging at high water.</obo:IAO_0000115>
        <oboInOwl:hasOBONamespace>GAZ</oboInOwl:hasOBONamespace>
        <oboInOwl:id>GAZ:00140680</oboInOwl:id>
        <rdfs:label>Vergilov Rocks</rdfs:label>
    </owl:NamedIndividual>
    


    <!-- http://purl.obolibrary.org/obo/GAZ_00140681 -->

    <owl:NamedIndividual rdf:about="http://purl.obolibrary.org/obo/GAZ_00140681">
        <obo:RO_0001025 rdf:resource="http://purl.obolibrary.org/obo/GAZ_00014113"/>
        <obo:IAO_0000115>The northwest extremity of Elephant Island, South Shetland Islands.</obo:IAO_0000115>
        <oboInOwl:hasOBONamespace>GAZ</oboInOwl:hasOBONamespace>
        <oboInOwl:id>GAZ:00140681</oboInOwl:id>
        <rdfs:label>Cape Yelcho</rdfs:label>
    </owl:NamedIndividual>
    


    <!-- http://purl.obolibrary.org/obo/GAZ_00140682 -->

    <owl:NamedIndividual rdf:about="http://purl.obolibrary.org/obo/GAZ_00140682">
        <obo:RO_0001025 rdf:resource="http://purl.obolibrary.org/obo/GAZ_00014113"/>
        <obo:IAO_0000115>A glacier at the W end of Elephant Island.</obo:IAO_0000115>
        <oboInOwl:hasOBONamespace>GAZ</oboInOwl:hasOBONamespace>
        <oboInOwl:id>GAZ:00140682</oboInOwl:id>
        <rdfs:label>Sultan Glacier</rdfs:label>
    </owl:NamedIndividual>
    


    <!-- http://purl.obolibrary.org/obo/GAZ_00140683 -->

    <owl:NamedIndividual rdf:about="http://purl.obolibrary.org/obo/GAZ_00140683">
        <obo:RO_0001025 rdf:resource="http://purl.obolibrary.org/obo/GAZ_00014113"/>
        <obo:IAO_0000115>A glacier on Elephant Island.</obo:IAO_0000115>
        <oboInOwl:hasOBONamespace>GAZ</oboInOwl:hasOBONamespace>
        <oboInOwl:id>GAZ:00140683</oboInOwl:id>
        <rdfs:label>Endurance Glacier</rdfs:label>
    </owl:NamedIndividual>
    


    <!-- http://purl.obolibrary.org/obo/GAZ_00140684 -->

    <owl:NamedIndividual rdf:about="http://purl.obolibrary.org/obo/GAZ_00140684">
        <obo:RO_0001025 rdf:resource="http://purl.obolibrary.org/obo/GAZ_00014113"/>
        <obo:IAO_0000115>The E cape of Elephant Island.</obo:IAO_0000115>
        <oboInOwl:hasOBONamespace>GAZ</oboInOwl:hasOBONamespace>
        <oboInOwl:id>GAZ:00140684</oboInOwl:id>
        <rdfs:label>Cape Valentine</rdfs:label>
    </owl:NamedIndividual>
    


    <!-- http://purl.obolibrary.org/obo/GAZ_00140685 -->

    <owl:NamedIndividual rdf:about="http://purl.obolibrary.org/obo/GAZ_00140685">
        <obo:RO_0001025 rdf:resource="http://purl.obolibrary.org/obo/GAZ_00014113"/>
        <obo:IAO_0000115>A ridge on the E end of Elephant Island.</obo:IAO_0000115>
        <oboInOwl:hasOBONamespace>GAZ</oboInOwl:hasOBONamespace>
        <oboInOwl:id>GAZ:00140685</oboInOwl:id>
        <rdfs:label>Pardo Ridge</rdfs:label>
    </owl:NamedIndividual>
    


    <!-- http://purl.obolibrary.org/obo/GAZ_00140686 -->

    <owl:NamedIndividual rdf:about="http://purl.obolibrary.org/obo/GAZ_00140686">
        <obo:RO_0001025 rdf:resource="http://purl.obolibrary.org/obo/GAZ_00014113"/>
        <obo:IAO_0000115>The most S cape of Elephant Island.</obo:IAO_0000115>
        <oboInOwl:hasOBONamespace>GAZ</oboInOwl:hasOBONamespace>
        <oboInOwl:id>GAZ:00140686</oboInOwl:id>
        <rdfs:label>Cape Lookout</rdfs:label>
    </owl:NamedIndividual>
    


    <!-- http://purl.obolibrary.org/obo/GAZ_00140687 -->

    <owl:NamedIndividual rdf:about="http://purl.obolibrary.org/obo/GAZ_00140687">
        <obo:RO_0001025 rdf:resource="http://purl.obolibrary.org/obo/GAZ_00014113"/>
        <obo:IAO_0000115>The most W cape of Elephant Island.</obo:IAO_0000115>
        <oboInOwl:hasOBONamespace>GAZ</oboInOwl:hasOBONamespace>
        <oboInOwl:id>GAZ:00140687</oboInOwl:id>
        <rdfs:label>Cape Lindsey</rdfs:label>
    </owl:NamedIndividual>
    


    <!-- http://purl.obolibrary.org/obo/GAZ_00140688 -->

    <owl:NamedIndividual rdf:about="http://purl.obolibrary.org/obo/GAZ_00140688">
        <obo:RO_0001025 rdf:resource="http://purl.obolibrary.org/obo/GAZ_00140059"/>
        <obo:IAO_0000115>A bay at the W end of Elephant Island.</obo:IAO_0000115>
        <oboInOwl:hasOBONamespace>GAZ</oboInOwl:hasOBONamespace>
        <oboInOwl:id>GAZ:00140688</oboInOwl:id>
        <rdfs:label>Table Bay</rdfs:label>
    </owl:NamedIndividual>
    


    <!-- http://purl.obolibrary.org/obo/GAZ_00140689 -->

    <owl:NamedIndividual rdf:about="http://purl.obolibrary.org/obo/GAZ_00140689">
        <obo:RO_0001025 rdf:resource="http://purl.obolibrary.org/obo/GAZ_00140059"/>
        <obo:IAO_0000115>A small bay, S of Cape Linsey, at the W of Elephant Island.</obo:IAO_0000115>
        <oboInOwl:hasOBONamespace>GAZ</oboInOwl:hasOBONamespace>
        <oboInOwl:id>GAZ:00140689</oboInOwl:id>
        <rdfs:label>Rodman Cove</rdfs:label>
    </owl:NamedIndividual>
    


    <!-- http://purl.obolibrary.org/obo/GAZ_00140690 -->

    <owl:NamedIndividual rdf:about="http://purl.obolibrary.org/obo/GAZ_00140690">
        <obo:RO_0001025 rdf:resource="http://purl.obolibrary.org/obo/GAZ_00140059"/>
        <obo:IAO_0000115>The 300 m wide cove indenting for 650 m the east coast of Greenwich Island, Antarctica south of Santa Cruz Point, and north of Parchevich Ridge.</obo:IAO_0000115>
        <oboInOwl:hasOBONamespace>GAZ</oboInOwl:hasOBONamespace>
        <oboInOwl:id>GAZ:00140690</oboInOwl:id>
        <rdfs:label>Gruev Cove</rdfs:label>
    </owl:NamedIndividual>
    


    <!-- http://purl.obolibrary.org/obo/GAZ_00140691 -->

    <owl:NamedIndividual rdf:about="http://purl.obolibrary.org/obo/GAZ_00140691">
        <obo:RO_0001025 rdf:resource="http://purl.obolibrary.org/obo/GAZ_00140059"/>
        <obo:IAO_0000115>A 1.5 km wide cove indenting for 900 m along the northern coast of Greenwich Island next E of Crutch Peaks, and NW of Sevtopolis Peak.</obo:IAO_0000115>
        <oboInOwl:hasOBONamespace>GAZ</oboInOwl:hasOBONamespace>
        <oboInOwl:id>GAZ:00140691</oboInOwl:id>
        <rdfs:label>Haskovo Cove</rdfs:label>
    </owl:NamedIndividual>
    


    <!-- http://purl.obolibrary.org/obo/GAZ_00140692 -->

    <owl:NamedIndividual rdf:about="http://purl.obolibrary.org/obo/GAZ_00140692">
        <obo:RO_0001025 rdf:resource="http://purl.obolibrary.org/obo/GAZ_00140059"/>
        <obo:IAO_0000115>A 1.8 km wide cove indenting for 1.2 km the north coast of Desolation Island between the two arms of that V-shaped island situated in the entrance to Hero Bay, Livingston Island, Antarctica.</obo:IAO_0000115>
        <oboInOwl:hasOBONamespace>GAZ</oboInOwl:hasOBONamespace>
        <oboInOwl:id>GAZ:00140692</oboInOwl:id>
        <rdfs:label>Kozma Cove</rdfs:label>
    </owl:NamedIndividual>
    


    <!-- http://purl.obolibrary.org/obo/GAZ_00140693 -->

    <owl:NamedIndividual rdf:about="http://purl.obolibrary.org/obo/GAZ_00140693">
        <obo:RO_0001025 rdf:resource="http://purl.obolibrary.org/obo/GAZ_00007328"/>
        <obo:IAO_0000115>A group of two small rocky islands, 500 by 370 m, and 350 by 200 m respectively, situated 300 m south of Iratais Point on Desolation Island off the north coast of Livingston Island, Antarctica. Separated from Desolation Island by Neck or Nothing Passage.</obo:IAO_0000115>
        <oboInOwl:hasOBONamespace>GAZ</oboInOwl:hasOBONamespace>
        <oboInOwl:id>GAZ:00140693</oboInOwl:id>
        <rdfs:label>Miladinovi Islets</rdfs:label>
    </owl:NamedIndividual>
    


    <!-- http://purl.obolibrary.org/obo/GAZ_00140694 -->

    <owl:NamedIndividual rdf:about="http://purl.obolibrary.org/obo/GAZ_00140694">
        <rdf:type rdf:resource="http://purl.obolibrary.org/obo/ENVO_00000029"/>
        <obo:RO_0001025 rdf:resource="http://purl.obolibrary.org/obo/GAZ_00140059"/>
        <obo:IAO_0000115>A narrow passage leading from Blythe Bay between the south end of Desolation Island and Miladinovi Islets, in the South Shetland Islands.</obo:IAO_0000115>
        <oboInOwl:hasOBONamespace>GAZ</oboInOwl:hasOBONamespace>
        <oboInOwl:id>GAZ:00140694</oboInOwl:id>
        <rdfs:label>Neck or Nothing Passage</rdfs:label>
    </owl:NamedIndividual>
    


    <!-- http://purl.obolibrary.org/obo/GAZ_00140695 -->

    <owl:NamedIndividual rdf:about="http://purl.obolibrary.org/obo/GAZ_00140695">
        <obo:RO_0001025 rdf:resource="http://purl.obolibrary.org/obo/GAZ_00140059"/>
        <obo:IAO_0000115>An anchorage at the southeast side of Desolation Island, lying north of Livingston Island in the South Shetland Islands.</obo:IAO_0000115>
        <oboInOwl:hasOBONamespace>GAZ</oboInOwl:hasOBONamespace>
        <oboInOwl:id>GAZ:00140695</oboInOwl:id>
        <rdfs:label>Blythe Bay</rdfs:label>
    </owl:NamedIndividual>
    


    <!-- http://purl.obolibrary.org/obo/GAZ_00140696 -->

    <owl:NamedIndividual rdf:about="http://purl.obolibrary.org/obo/GAZ_00140696">
        <obo:RO_0001025 rdf:resource="http://purl.obolibrary.org/obo/GAZ_00140695"/>
        <obo:IAO_0000115>A two km wide cove in the north coast of Greenwich Island, Antarctica. It is bounded by Archar Peninsula to the south, and Express Island to the northeast. The Cove is entered between Duff Point and the northern extremity of Express Island.</obo:IAO_0000115>
        <oboInOwl:hasOBONamespace>GAZ</oboInOwl:hasOBONamespace>
        <oboInOwl:id>GAZ:00140696</oboInOwl:id>
        <rdfs:label>Razlog Cove</rdfs:label>
    </owl:NamedIndividual>
    


    <!-- http://purl.obolibrary.org/obo/GAZ_00140697 -->

    <owl:NamedIndividual rdf:about="http://purl.obolibrary.org/obo/GAZ_00140697">
        <obo:RO_0001025 rdf:resource="http://purl.obolibrary.org/obo/GAZ_00007328"/>
        <obo:IAO_0000115>A narrow craggy island, 1.0 km long, lying close offshore of northwest Greenwich Island, due north of Greaves Peak.</obo:IAO_0000115>
        <oboInOwl:hasOBONamespace>GAZ</oboInOwl:hasOBONamespace>
        <oboInOwl:id>GAZ:00140697</oboInOwl:id>
        <rdfs:label>Express Island</rdfs:label>
    </owl:NamedIndividual>
    


    <!-- http://purl.obolibrary.org/obo/GAZ_00140698 -->

    <owl:NamedIndividual rdf:about="http://purl.obolibrary.org/obo/GAZ_00140698">
        <obo:RO_0001025 rdf:resource="http://purl.obolibrary.org/obo/GAZ_00140059"/>
        <obo:IAO_0000115>A small harbor entered between Glacier Bluff and Spit Point, indenting the southwest side of Greenwich Island in the South Shetland Islands.</obo:IAO_0000115>
        <oboInOwl:hasOBONamespace>GAZ</oboInOwl:hasOBONamespace>
        <oboInOwl:id>GAZ:00140698</oboInOwl:id>
        <rdfs:label>Yankee Harbour</rdfs:label>
    </owl:NamedIndividual>
    


    <!-- http://purl.obolibrary.org/obo/GAZ_00140699 -->

    <owl:NamedIndividual rdf:about="http://purl.obolibrary.org/obo/GAZ_00140699">
        <obo:RO_0001025 rdf:resource="http://purl.obolibrary.org/obo/GAZ_00140059"/>
        <obo:IAO_0000115>A 2.6 km wide cove indenting for 1.5 km the SW coast of Greenwich Island, Antarctica, between Triangle Point and the westernmost extremity of the moraine spit protecting Yankee Harbour.</obo:IAO_0000115>
        <oboInOwl:hasOBONamespace>GAZ</oboInOwl:hasOBONamespace>
        <oboInOwl:id>GAZ:00140699</oboInOwl:id>
        <rdfs:label>Shopski Cove</rdfs:label>
    </owl:NamedIndividual>
    


    <!-- http://purl.obolibrary.org/obo/GAZ_00140700 -->

    <owl:NamedIndividual rdf:about="http://purl.obolibrary.org/obo/GAZ_00140700">
        <obo:RO_0001025 rdf:resource="http://purl.obolibrary.org/obo/GAZ_00140059"/>
        <obo:IAO_0000115>A 1.8 km wide cove indenting for 600 m the N coast of Greenwich Island, Antarctica, NW of Mount Plymouth, and NE of Sevtopolis Peak.</obo:IAO_0000115>
        <oboInOwl:hasOBONamespace>GAZ</oboInOwl:hasOBONamespace>
        <oboInOwl:id>GAZ:00140700</oboInOwl:id>
        <rdfs:label>Skaptopara Cove</rdfs:label>
    </owl:NamedIndividual>
    


    <!-- http://purl.obolibrary.org/obo/GAZ_00140701 -->

    <owl:NamedIndividual rdf:about="http://purl.obolibrary.org/obo/GAZ_00140701">
        <rdf:type rdf:resource="http://purl.obolibrary.org/obo/ENVO_00000305"/>
        <obo:RO_0001025 rdf:resource="http://purl.obolibrary.org/obo/GAZ_00017735"/>
        <obo:IAO_0000115>A headland on the north coast of Greenwich Island, Antarctica situated 6.9 km east of Duff Point, 2.1 km east-southeast of Kabile Island, 2.2 km east-northeast of Crutch Peaks, 1.8 km south of Ongley Island, 5.5 km west of Aguedo Point, and 2.3 km north-northwest of Sevtopolis Peak. Forming the east side of the entrance to Haskovo Cove.</obo:IAO_0000115>
        <oboInOwl:hasOBONamespace>GAZ</oboInOwl:hasOBONamespace>
        <oboInOwl:id>GAZ:00140701</oboInOwl:id>
        <rdfs:label>Aprilov Point</rdfs:label>
    </owl:NamedIndividual>
    


    <!-- http://purl.obolibrary.org/obo/GAZ_00140702 -->

    <owl:NamedIndividual rdf:about="http://purl.obolibrary.org/obo/GAZ_00140702">
        <obo:RO_0001025 rdf:resource="http://purl.obolibrary.org/obo/GAZ_00140701"/>
        <obo:IAO_0000115>A peninsula located in the North-Western extremity of Greenwich Island, Antarctica. The three km long peninsula is bounded by Razlog Cove to the North and McFarlane Strait to the South.</obo:IAO_0000115>
        <oboInOwl:hasOBONamespace>GAZ</oboInOwl:hasOBONamespace>
        <oboInOwl:id>GAZ:00140702</oboInOwl:id>
        <rdfs:label>Archar Peninsula</rdfs:label>
    </owl:NamedIndividual>
    


    <!-- http://purl.obolibrary.org/obo/GAZ_00140703 -->

    <owl:NamedIndividual rdf:about="http://purl.obolibrary.org/obo/GAZ_00140703">
        <obo:RO_0001025 rdf:resource="http://purl.obolibrary.org/obo/GAZ_00140051"/>
        <obo:IAO_0000115>A rocky peak of elevation 450 m projecting from the ice cap of Greenwich Island in the northeast extremity of Breznik Heights. Situated 1 km west-southwest of Bogdan Ridge, and 600 m north of Parchevich Ridge. Overlooking Gruev Cove to the east.</obo:IAO_0000115>
        <oboInOwl:hasOBONamespace>GAZ</oboInOwl:hasOBONamespace>
        <oboInOwl:id>GAZ:00140703</oboInOwl:id>
        <rdfs:label>Benkovski Nunatak</rdfs:label>
    </owl:NamedIndividual>
    


    <!-- http://purl.obolibrary.org/obo/GAZ_00140704 -->

    <owl:NamedIndividual rdf:about="http://purl.obolibrary.org/obo/GAZ_00140704">
        <rdf:type rdf:resource="http://purl.obolibrary.org/obo/ENVO_00000305"/>
        <obo:RO_0001025 rdf:resource="http://purl.obolibrary.org/obo/GAZ_00007288"/>
        <obo:IAO_0000115>A headland on the southwest coast of Robert Island, Antarctica situated 4.5 km southeast of Negra Point, 1.7 km west of Bajo Nunatak, 1.8 km west-northwest of Zahari Point, and 3.7 km northwest of Edwards Point, as well as 5 km northeast of Ash Point on Greenwich Island.</obo:IAO_0000115>
        <oboInOwl:hasOBONamespace>GAZ</oboInOwl:hasOBONamespace>
        <oboInOwl:id>GAZ:00140704</oboInOwl:id>
        <rdfs:label>Beron Point</rdfs:label>
    </owl:NamedIndividual>
    


    <!-- http://purl.obolibrary.org/obo/GAZ_00140705 -->

    <owl:NamedIndividual rdf:about="http://purl.obolibrary.org/obo/GAZ_00140705">
        <rdf:type rdf:resource="http://purl.obolibrary.org/obo/ENVO_00000305"/>
        <obo:RO_0001025 rdf:resource="http://purl.obolibrary.org/obo/GAZ_00007329"/>
        <obo:IAO_0000115>A headland on the coast of Moon Bay, Livingston Island, Antarctica situated 5.7 km south-southwest of Edinburgh Hill, 8.3 km southeast of Miziya Peak, 4 km east by north of Sliven Peak, 3.1 km northeast of Zlatograd Rock, and 5 km northwest of Rila Point.</obo:IAO_0000115>
        <oboInOwl:hasOBONamespace>GAZ</oboInOwl:hasOBONamespace>
        <oboInOwl:id>GAZ:00140705</oboInOwl:id>
        <rdfs:label>Elemag Point</rdfs:label>
    </owl:NamedIndividual>
    


    <!-- http://purl.obolibrary.org/obo/GAZ_00140706 -->

    <owl:NamedIndividual rdf:about="http://purl.obolibrary.org/obo/GAZ_00140706">
        <obo:RO_0001025 rdf:resource="http://purl.obolibrary.org/obo/GAZ_00017735"/>
        <obo:IAO_0000115>A 160m rocky peak on the North coast of Greenwich Island.</obo:IAO_0000115>
        <oboInOwl:hasOBONamespace>GAZ</oboInOwl:hasOBONamespace>
        <oboInOwl:id>GAZ:00140706</oboInOwl:id>
        <rdfs:label>Hrabar Nunatak</rdfs:label>
    </owl:NamedIndividual>
    


    <!-- http://purl.obolibrary.org/obo/GAZ_00140707 -->

    <owl:NamedIndividual rdf:about="http://purl.obolibrary.org/obo/GAZ_00140707">
        <obo:RO_0001025 rdf:resource="http://purl.obolibrary.org/obo/GAZ_00007288"/>
        <obo:IAO_0000115>A 1.5-km long peninsula forming the south extremity of Robert Island, Antarctica. Bounded by Micalvi Cove to the northwest, and Bransfield Strait to the southeast.</obo:IAO_0000115>
        <oboInOwl:hasOBONamespace>GAZ</oboInOwl:hasOBONamespace>
        <oboInOwl:id>GAZ:00140707</oboInOwl:id>
        <rdfs:label>Kermen Peninsula</rdfs:label>
    </owl:NamedIndividual>
    


    <!-- http://purl.obolibrary.org/obo/GAZ_00140708 -->

    <owl:NamedIndividual rdf:about="http://purl.obolibrary.org/obo/GAZ_00140708">
        <obo:RO_0001025 rdf:resource="http://purl.obolibrary.org/obo/GAZ_00017735"/>
        <obo:IAO_0000115>A glacier on Greenwich Island to the south of Greaves Peak and Crutch Peak and to the west of Lloyd hill. The glacier drains westwards into McFarlane Strait and extends 2.5km inland. It has a width of 5km.</obo:IAO_0000115>
        <oboInOwl:hasOBONamespace>GAZ</oboInOwl:hasOBONamespace>
        <oboInOwl:id>GAZ:00140708</oboInOwl:id>
        <rdfs:label>Yakoruda Glacier</rdfs:label>
    </owl:NamedIndividual>
    


    <!-- http://purl.obolibrary.org/obo/GAZ_00140709 -->

    <owl:NamedIndividual rdf:about="http://purl.obolibrary.org/obo/GAZ_00140709">
        <obo:RO_0001025 rdf:resource="http://purl.obolibrary.org/obo/GAZ_00140708"/>
        <obo:IAO_0000115>A rocky hill of elevation 90 m projecting from Yakoruda Glacier, Greenwich Island.</obo:IAO_0000115>
        <oboInOwl:hasOBONamespace>GAZ</oboInOwl:hasOBONamespace>
        <oboInOwl:id>GAZ:00140709</oboInOwl:id>
        <rdfs:label>Kerseblept Nunatak</rdfs:label>
    </owl:NamedIndividual>
    


    <!-- http://purl.obolibrary.org/obo/GAZ_00140710 -->

    <owl:NamedIndividual rdf:about="http://purl.obolibrary.org/obo/GAZ_00140710">
        <obo:RO_0001025 rdf:resource="http://purl.obolibrary.org/obo/GAZ_00139976"/>
        <obo:IAO_0000115>A conspicuous rocky peak of elevation 290 m projecting from Murgash Glacier, Greenwich Island.</obo:IAO_0000115>
        <oboInOwl:hasOBONamespace>GAZ</oboInOwl:hasOBONamespace>
        <oboInOwl:id>GAZ:00140710</oboInOwl:id>
        <rdfs:label>Kotrag Nunatak</rdfs:label>
    </owl:NamedIndividual>
    


    <!-- http://purl.obolibrary.org/obo/GAZ_00140711 -->

    <owl:NamedIndividual rdf:about="http://purl.obolibrary.org/obo/GAZ_00140711">
        <obo:RO_0001025 rdf:resource="http://purl.obolibrary.org/obo/GAZ_00140051"/>
        <obo:IAO_0000115>A rocky peak of elevation 430 m projecting from the ice cap in Breznik Heights on Greenwich Island, Antarctica.</obo:IAO_0000115>
        <oboInOwl:hasOBONamespace>GAZ</oboInOwl:hasOBONamespace>
        <oboInOwl:id>GAZ:00140711</oboInOwl:id>
        <rdfs:label>Lyutitsa Nunatak</rdfs:label>
    </owl:NamedIndividual>
    


    <!-- http://purl.obolibrary.org/obo/GAZ_00140712 -->

    <owl:NamedIndividual rdf:about="http://purl.obolibrary.org/obo/GAZ_00140712">
        <obo:RO_0001025 rdf:resource="http://purl.obolibrary.org/obo/GAZ_00017735"/>
        <obo:IAO_0000115>A glacier on Greenwich Island is bounded by Vratsa Peak to the SW, central Breznik Heights to the W, and a low ridge bordering Hardy Cove to the NE. It extends 3.7 km in E-W direction, and 2 km in N-S direction and drains eastwards into Bransfield Strait north of Fort Point.</obo:IAO_0000115>
        <oboInOwl:hasOBONamespace>GAZ</oboInOwl:hasOBONamespace>
        <oboInOwl:id>GAZ:00140712</oboInOwl:id>
        <rdfs:label>Musala Glacier</rdfs:label>
    </owl:NamedIndividual>
    


    <!-- http://purl.obolibrary.org/obo/GAZ_00140713 -->

    <owl:NamedIndividual rdf:about="http://purl.obolibrary.org/obo/GAZ_00140713">
        <obo:RO_0001025 rdf:resource="http://purl.obolibrary.org/obo/GAZ_00140708"/>
        <obo:IAO_0000115>A rocky peak of elevation 150 m projecting from Yakoruda Glacier, Greenwich Island, Antarctica.</obo:IAO_0000115>
        <oboInOwl:hasOBONamespace>GAZ</oboInOwl:hasOBONamespace>
        <oboInOwl:id>GAZ:00140713</oboInOwl:id>
        <rdfs:label>Panagyurishte Nunatak</rdfs:label>
    </owl:NamedIndividual>
    


    <!-- http://purl.obolibrary.org/obo/GAZ_00140714 -->

    <owl:NamedIndividual rdf:about="http://purl.obolibrary.org/obo/GAZ_00140714">
        <obo:RO_0001025 rdf:resource="http://purl.obolibrary.org/obo/GAZ_00139801"/>
        <obo:IAO_0000115>An ice-free point on the northeast coast of Varna Peninsula, Livingston Island, Antarctica forming the northwest side of the entrance to Dragon Cove. Situated 1.1 km south-southeast of Williams Point, 750 m northeast of Sayer Nunatak, and 800 m west-northwest of Ficheto Point.</obo:IAO_0000115>
        <oboInOwl:hasOBONamespace>GAZ</oboInOwl:hasOBONamespace>
        <oboInOwl:id>GAZ:00140714</oboInOwl:id>
        <rdfs:label>Sigritsa Point</rdfs:label>
    </owl:NamedIndividual>
    


    <!-- http://purl.obolibrary.org/obo/GAZ_00140715 -->

    <owl:NamedIndividual rdf:about="http://purl.obolibrary.org/obo/GAZ_00140715">
        <obo:RO_0001025 rdf:resource="http://purl.obolibrary.org/obo/GAZ_00017735"/>
        <obo:IAO_0000115>A glacier on Greenwich Island, Antarctica. The glacier is bounded by Razgrad Peak to the west, Momchil Peak to the north, and Viskyar Ridge to the east. The glacier extends 2 km in the east-west direction, and 1.8 km in the north-south direction. It drains southwards into McFarlane Strait between Ephraim Bluff and Sartorius Point.</obo:IAO_0000115>
        <oboInOwl:hasOBONamespace>GAZ</oboInOwl:hasOBONamespace>
        <oboInOwl:id>GAZ:00140715</oboInOwl:id>
        <rdfs:label>Zheravna Glacier</rdfs:label>
    </owl:NamedIndividual>
    


    <!-- http://purl.obolibrary.org/obo/GAZ_00140716 -->

    <owl:NamedIndividual rdf:about="http://purl.obolibrary.org/obo/GAZ_00140716">
        <obo:RO_0001025 rdf:resource="http://purl.obolibrary.org/obo/GAZ_00140016"/>
        <obo:IAO_0000115>A sharp peak rising to 550 m in the Eastern extremity of Bowles Ridge, Livingston Island, Antarctica. The peak sumounts the Huron Glacier to the South and East and Struma Glacier to the North.</obo:IAO_0000115>
        <oboInOwl:hasOBONamespace>GAZ</oboInOwl:hasOBONamespace>
        <oboInOwl:id>GAZ:00140716</oboInOwl:id>
        <rdfs:label>Atanasoff Nunatak</rdfs:label>
    </owl:NamedIndividual>
    


    <!-- http://purl.obolibrary.org/obo/GAZ_00140717 -->

    <owl:NamedIndividual rdf:about="http://purl.obolibrary.org/obo/GAZ_00140717">
        <obo:RO_0001025 rdf:resource="http://purl.obolibrary.org/obo/GAZ_00007330"/>
        <obo:IAO_0000115>A series of beaches which extend for 11 km along the broad western end of Byers Peninsula, Livingston Island, in the South Shetland Islands.</obo:IAO_0000115>
        <oboInOwl:hasOBONamespace>GAZ</oboInOwl:hasOBONamespace>
        <oboInOwl:id>GAZ:00140717</oboInOwl:id>
        <rdfs:label>President Beaches</rdfs:label>
    </owl:NamedIndividual>
    


    <!-- http://purl.obolibrary.org/obo/GAZ_00140718 -->

    <owl:NamedIndividual rdf:about="http://purl.obolibrary.org/obo/GAZ_00140718">
        <obo:RO_0001025 rdf:resource="http://purl.obolibrary.org/obo/GAZ_00004045"/>
        <obo:IAO_0000115>An undersea canyon in the Weddell Sea.</obo:IAO_0000115>
        <oboInOwl:hasOBONamespace>GAZ</oboInOwl:hasOBONamespace>
        <oboInOwl:id>GAZ:00140718</oboInOwl:id>
        <rdfs:label>Akademik Federov Canyon</rdfs:label>
    </owl:NamedIndividual>
    


    <!-- http://purl.obolibrary.org/obo/GAZ_00140737 -->

    <owl:NamedIndividual rdf:about="http://purl.obolibrary.org/obo/GAZ_00140737">
        <obo:RO_0001025 rdf:resource="http://purl.obolibrary.org/obo/GAZ_00023319"/>
        <obo:IAO_0000115>Anice-filled cirque, or corrie, close north of Amphibolite Point on the south coast of Coronation Island.</obo:IAO_0000115>
        <oboInOwl:hasOBONamespace>GAZ</oboInOwl:hasOBONamespace>
        <oboInOwl:id>GAZ:00140737</oboInOwl:id>
        <rdfs:label>Avalanche Corrie</rdfs:label>
    </owl:NamedIndividual>
    


    <!-- http://purl.obolibrary.org/obo/GAZ_00140744 -->

    <owl:NamedIndividual rdf:about="http://purl.obolibrary.org/obo/GAZ_00140744">
        <obo:RO_0001025 rdf:resource="http://purl.obolibrary.org/obo/GAZ_00014088"/>
        <obo:IAO_0000115>An ice-covered area (essentially a glacial cirque) enclosed on three sides by rock ridges, but open to the south, lying between Mount Umbriel and Venus Glacier in eastern Alexander Island.</obo:IAO_0000115>
        <oboInOwl:hasOBONamespace>GAZ</oboInOwl:hasOBONamespace>
        <oboInOwl:id>GAZ:00140744</oboInOwl:id>
        <rdfs:label>The Quadrangle</rdfs:label>
    </owl:NamedIndividual>
    


    <!-- http://purl.obolibrary.org/obo/GAZ_00140745 -->

    <owl:NamedIndividual rdf:about="http://purl.obolibrary.org/obo/GAZ_00140745">
        <obo:RO_0001025 rdf:resource="http://purl.obolibrary.org/obo/GAZ_00014088"/>
        <obo:IAO_0000115>A glacier on the E coast of Alexander Island, 10 mi long and 6 mi wide at its mouth flowing E into George VI Sound between Keystone Cliffs and Triton Point.</obo:IAO_0000115>
        <oboInOwl:hasOBONamespace>GAZ</oboInOwl:hasOBONamespace>
        <oboInOwl:id>GAZ:00140745</oboInOwl:id>
        <rdfs:label>Venus Glacier</rdfs:label>
    </owl:NamedIndividual>
    


    <!-- http://purl.obolibrary.org/obo/GAZ_00140748 -->

    <owl:NamedIndividual rdf:about="http://purl.obolibrary.org/obo/GAZ_00140748">
        <obo:RO_0001025 rdf:resource="http://purl.obolibrary.org/obo/GAZ_00141024"/>
        <obo:IAO_0000115>A cove which lies immediately northeast of Cape Whitson, along the south coast of Laurie Island in the South Orkney Islands.</obo:IAO_0000115>
        <oboInOwl:hasOBONamespace>GAZ</oboInOwl:hasOBONamespace>
        <oboInOwl:id>GAZ:00140748</oboInOwl:id>
        <rdfs:label>Aitken Cove</rdfs:label>
    </owl:NamedIndividual>
    


    <!-- http://purl.obolibrary.org/obo/GAZ_00140749 -->

    <owl:NamedIndividual rdf:about="http://purl.obolibrary.org/obo/GAZ_00140749">
        <obo:RO_0001025 rdf:resource="http://purl.obolibrary.org/obo/GAZ_00141554"/>
        <obo:IAO_0000115>A bare rock island nearly 1 mi long, lying just off the north-central side of Schirmacher Hills, Queen Maud Land.</obo:IAO_0000115>
        <oboInOwl:hasOBONamespace>GAZ</oboInOwl:hasOBONamespace>
        <oboInOwl:id>GAZ:00140749</oboInOwl:id>
        <rdfs:label>Nadezhdy Island</rdfs:label>
    </owl:NamedIndividual>
    


    <!-- http://purl.obolibrary.org/obo/GAZ_00140750 -->

    <owl:NamedIndividual rdf:about="http://purl.obolibrary.org/obo/GAZ_00140750">
        <obo:RO_0001025 rdf:resource="http://purl.obolibrary.org/obo/GAZ_00141554"/>
        <obo:IAO_0000115>A small cove 4.8 km east-southeast of Nadezhdy Island, indenting the north side of the Schirmacher Hills, Queen Maud Land.</obo:IAO_0000115>
        <oboInOwl:hasOBONamespace>GAZ</oboInOwl:hasOBONamespace>
        <oboInOwl:id>GAZ:00140750</oboInOwl:id>
        <rdfs:label>Akkuratnaya Cove</rdfs:label>
    </owl:NamedIndividual>
    


    <!-- http://purl.obolibrary.org/obo/GAZ_00140751 -->

    <owl:NamedIndividual rdf:about="http://purl.obolibrary.org/obo/GAZ_00140751">
        <obo:RO_0001025 rdf:resource="http://purl.obolibrary.org/obo/GAZ_00007426"/>
        <obo:IAO_0000115>A small cove at the southeast side of Point Thomas in Admiralty Bay, King George Island.</obo:IAO_0000115>
        <oboInOwl:hasOBONamespace>GAZ</oboInOwl:hasOBONamespace>
        <oboInOwl:id>GAZ:00140751</oboInOwl:id>
        <rdfs:label>Arctowski Cove</rdfs:label>
    </owl:NamedIndividual>
    


    <!-- http://purl.obolibrary.org/obo/GAZ_00140753 -->

    <owl:NamedIndividual rdf:about="http://purl.obolibrary.org/obo/GAZ_00140753">
        <obo:RO_0001025 rdf:resource="http://purl.obolibrary.org/obo/GAZ_00141552"/>
        <obo:IAO_0000115>A large bay lying between Capes Renard and Willems, along the west coast of Graham Land.</obo:IAO_0000115>
        <oboInOwl:hasOBONamespace>GAZ</oboInOwl:hasOBONamespace>
        <oboInOwl:id>GAZ:00140753</oboInOwl:id>
        <rdfs:label>Flandres Bay</rdfs:label>
    </owl:NamedIndividual>
    


    <!-- http://purl.obolibrary.org/obo/GAZ_00140754 -->

    <owl:NamedIndividual rdf:about="http://purl.obolibrary.org/obo/GAZ_00140754">
        <obo:RO_0001025 rdf:resource="http://purl.obolibrary.org/obo/GAZ_00140753"/>
        <obo:IAO_0000115>A cove 1.6 km long, lying just east of Cangrejo Cove in the southwest part of Flandres Bay, on the west coast of Graham Land.</obo:IAO_0000115>
        <oboInOwl:hasOBONamespace>GAZ</oboInOwl:hasOBONamespace>
        <oboInOwl:id>GAZ:00140754</oboInOwl:id>
        <rdfs:label>Azure Cove</rdfs:label>
    </owl:NamedIndividual>
    


    <!-- http://purl.obolibrary.org/obo/GAZ_00140755 -->

    <owl:NamedIndividual rdf:about="http://purl.obolibrary.org/obo/GAZ_00140755">
        <obo:RO_0001025 rdf:resource="http://purl.obolibrary.org/obo/GAZ_00140753"/>
        <obo:IAO_0000115>A cove 1.5 miles long lying immediately west of Azure Cove in Flandres Bay, along the west coast of Graham Land.</obo:IAO_0000115>
        <oboInOwl:hasOBONamespace>GAZ</oboInOwl:hasOBONamespace>
        <oboInOwl:id>GAZ:00140755</oboInOwl:id>
        <rdfs:label>Cangrejo Cove</rdfs:label>
    </owl:NamedIndividual>
    


    <!-- http://purl.obolibrary.org/obo/GAZ_00140757 -->

    <owl:NamedIndividual rdf:about="http://purl.obolibrary.org/obo/GAZ_00140757">
        <obo:RO_0001025 rdf:resource="http://purl.obolibrary.org/obo/GAZ_00141554"/>
        <obo:IAO_0000115>A cove indenting the north side of Hahellerskarvet in the Muhlig-Hofmann Mountains, Queen Maud Land.</obo:IAO_0000115>
        <oboInOwl:hasOBONamespace>GAZ</oboInOwl:hasOBONamespace>
        <oboInOwl:id>GAZ:00140757</oboInOwl:id>
        <rdfs:label>Hahelleren Cove</rdfs:label>
    </owl:NamedIndividual>
    


    <!-- http://purl.obolibrary.org/obo/GAZ_00140758 -->

    <owl:NamedIndividual rdf:about="http://purl.obolibrary.org/obo/GAZ_00140758">
        <obo:RO_0001025 rdf:resource="http://purl.obolibrary.org/obo/GAZ_00140014"/>
        <obo:IAO_0000115>A cove on the east side of False Bay, Livingston Island, in the South Shetland Islands.</obo:IAO_0000115>
        <oboInOwl:hasOBONamespace>GAZ</oboInOwl:hasOBONamespace>
        <oboInOwl:id>GAZ:00140758</oboInOwl:id>
        <rdfs:label>Inepta Cove</rdfs:label>
    </owl:NamedIndividual>
    


    <!-- http://purl.obolibrary.org/obo/GAZ_00140759 -->

    <owl:NamedIndividual rdf:about="http://purl.obolibrary.org/obo/GAZ_00140759">
        <obo:RO_0001025 rdf:resource="http://purl.obolibrary.org/obo/GAZ_00139453"/>
        <obo:IAO_0000115>A small cove in the east side of Discovery Bay, Greenwich Island, South Shetland Islands. The cove is immediately adjacent to the Arturo Prat Station on Guesalaga Peninsula.</obo:IAO_0000115>
        <oboInOwl:hasOBONamespace>GAZ</oboInOwl:hasOBONamespace>
        <oboInOwl:id>GAZ:00140759</oboInOwl:id>
        <rdfs:label>Iquique Cove</rdfs:label>
    </owl:NamedIndividual>
    


    <!-- http://purl.obolibrary.org/obo/GAZ_00140760 -->

    <owl:NamedIndividual rdf:about="http://purl.obolibrary.org/obo/GAZ_00140760">
        <obo:RO_0001025 rdf:resource="http://purl.obolibrary.org/obo/GAZ_00140365"/>
        <obo:IAO_0000115>A bay, 6 km wide, lying at the east side of Cape Klovstad where it forms the head of Robertson Bay, northern Victoria Land.</obo:IAO_0000115>
        <oboInOwl:hasOBONamespace>GAZ</oboInOwl:hasOBONamespace>
        <oboInOwl:id>GAZ:00140760</oboInOwl:id>
        <rdfs:label>Protection Cove</rdfs:label>
    </owl:NamedIndividual>
    


    <!-- http://purl.obolibrary.org/obo/GAZ_00140761 -->

    <owl:NamedIndividual rdf:about="http://purl.obolibrary.org/obo/GAZ_00140761">
        <obo:RO_0001025 rdf:resource="http://purl.obolibrary.org/obo/GAZ_00139950"/>
        <obo:IAO_0000115>A cove bounded by ice cliffs which lies at the foot of Remus Glacier in the southeast corner of Neny Fjord, along the west coast of Graham Land.</obo:IAO_0000115>
        <oboInOwl:hasOBONamespace>GAZ</oboInOwl:hasOBONamespace>
        <oboInOwl:id>GAZ:00140761</oboInOwl:id>
        <rdfs:label>Providence Cove</rdfs:label>
    </owl:NamedIndividual>
    


    <!-- http://purl.obolibrary.org/obo/GAZ_00140763 -->

    <owl:NamedIndividual rdf:about="http://purl.obolibrary.org/obo/GAZ_00140763">
        <obo:RO_0001025 rdf:resource="http://purl.obolibrary.org/obo/GAZ_00141024"/>
        <obo:IAO_0000115>A cove in the southwest part of Jessie Bay on the north coast of Laurie Island, in the South Orkney Islands.</obo:IAO_0000115>
        <oboInOwl:hasOBONamespace>GAZ</oboInOwl:hasOBONamespace>
        <oboInOwl:id>GAZ:00140763</oboInOwl:id>
        <rdfs:label>Sheila Cove</rdfs:label>
    </owl:NamedIndividual>
    


    <!-- http://purl.obolibrary.org/obo/GAZ_00140764 -->

    <owl:NamedIndividual rdf:about="http://purl.obolibrary.org/obo/GAZ_00140764">
        <obo:RO_0001025 rdf:resource="http://purl.obolibrary.org/obo/GAZ_00140090"/>
        <obo:IAO_0000115>A small coastal indentation on the north shore of Prince Gustav Channel, between Chapel Hill and Church Point, Trinity Peninsula.</obo:IAO_0000115>
        <oboInOwl:hasOBONamespace>GAZ</oboInOwl:hasOBONamespace>
        <oboInOwl:id>GAZ:00140764</oboInOwl:id>
        <rdfs:label>Shelter Cove</rdfs:label>
    </owl:NamedIndividual>
    


    <!-- http://purl.obolibrary.org/obo/GAZ_00140765 -->

    <owl:NamedIndividual rdf:about="http://purl.obolibrary.org/obo/GAZ_00140765">
        <obo:RO_0001025 rdf:resource="http://purl.obolibrary.org/obo/GAZ_00004045"/>
        <obo:IAO_0000115>A bay 4.8 km wide, which indents the south coast of Coronation Island between Cape Hansen and Olivine Point, in the South Orkney Islands.</obo:IAO_0000115>
        <oboInOwl:hasOBONamespace>GAZ</oboInOwl:hasOBONamespace>
        <oboInOwl:id>GAZ:00140765</oboInOwl:id>
        <rdfs:label>Iceberg Bay</rdfs:label>
    </owl:NamedIndividual>
    


    <!-- http://purl.obolibrary.org/obo/GAZ_00140766 -->

    <owl:NamedIndividual rdf:about="http://purl.obolibrary.org/obo/GAZ_00140766">
        <obo:RO_0001025 rdf:resource="http://purl.obolibrary.org/obo/GAZ_00140765"/>
        <obo:IAO_0000115>A small sheltered cove in the northwest corner of Iceberg Bay on the south coast of Coronation Island, in the South Orkney Islands.</obo:IAO_0000115>
        <oboInOwl:hasOBONamespace>GAZ</oboInOwl:hasOBONamespace>
        <oboInOwl:id>GAZ:00140766</oboInOwl:id>
        <rdfs:label>Shingle Cove</rdfs:label>
    </owl:NamedIndividual>
    


    <!-- http://purl.obolibrary.org/obo/GAZ_00140767 -->

    <owl:NamedIndividual rdf:about="http://purl.obolibrary.org/obo/GAZ_00140767">
        <obo:RO_0001025 rdf:resource="http://purl.obolibrary.org/obo/GAZ_00004045"/>
        <obo:IAO_0000115>An ice-filled inlet, nurtured by several NE and E flowing glaciers, lying between Rock Pile Peaks and Hollick-Kenyon Peninsula along the E coast of Antarctic Peninsula.</obo:IAO_0000115>
        <oboInOwl:hasOBONamespace>GAZ</oboInOwl:hasOBONamespace>
        <oboInOwl:id>GAZ:00140767</oboInOwl:id>
        <rdfs:label>Mobiloil Inlet</rdfs:label>
    </owl:NamedIndividual>
    


    <!-- http://purl.obolibrary.org/obo/GAZ_00140796 -->

    <owl:NamedIndividual rdf:about="http://purl.obolibrary.org/obo/GAZ_00140796">
        <obo:RO_0001025 rdf:resource="http://purl.obolibrary.org/obo/GAZ_00051499"/>
        <obo:IAO_0000115>A minor undersea basin, almost an appendage to the Southeast Pacific Basin.</obo:IAO_0000115>
        <oboInOwl:hasOBONamespace>GAZ</oboInOwl:hasOBONamespace>
        <oboInOwl:id>GAZ:00140796</oboInOwl:id>
        <rdfs:label>Balleny Basin</rdfs:label>
    </owl:NamedIndividual>
    


    <!-- http://purl.obolibrary.org/obo/GAZ_00140797 -->

    <owl:NamedIndividual rdf:about="http://purl.obolibrary.org/obo/GAZ_00140797">
        <obo:RO_0001025 rdf:resource="http://purl.obolibrary.org/obo/GAZ_00140796"/>
        <obo:IAO_0000115>The seamounts in Balleny Basin named in association with Adare Peninsula and Cape Adare.</obo:IAO_0000115>
        <oboInOwl:hasOBONamespace>GAZ</oboInOwl:hasOBONamespace>
        <oboInOwl:id>GAZ:00140797</oboInOwl:id>
        <rdfs:label>Adare Seamounts</rdfs:label>
    </owl:NamedIndividual>
    


    <!-- http://purl.obolibrary.org/obo/GAZ_00140800 -->

    <owl:NamedIndividual rdf:about="http://purl.obolibrary.org/obo/GAZ_00140800">
        <obo:RO_0001025 rdf:resource="http://purl.obolibrary.org/obo/GAZ_00004045"/>
        <obo:IAO_0000115>A bank in the Weddell Sea.</obo:IAO_0000115>
        <oboInOwl:hasOBONamespace>GAZ</oboInOwl:hasOBONamespace>
        <oboInOwl:id>GAZ:00140800</oboInOwl:id>
        <rdfs:label>Albert Bank</rdfs:label>
    </owl:NamedIndividual>
    


    <!-- http://purl.obolibrary.org/obo/GAZ_00140812 -->

    <owl:NamedIndividual rdf:about="http://purl.obolibrary.org/obo/GAZ_00140812">
        <rdf:type rdf:resource="http://purl.obolibrary.org/obo/ENVO_00000275"/>
        <obo:RO_0001025 rdf:resource="http://purl.obolibrary.org/obo/GAZ_00023304"/>
        <obo:IAO_0000115>An undersea trough.</obo:IAO_0000115>
        <oboInOwl:hasOBONamespace>GAZ</oboInOwl:hasOBONamespace>
        <oboInOwl:id>GAZ:00140812</oboInOwl:id>
        <rdfs:label>Adare Trough</rdfs:label>
    </owl:NamedIndividual>
    


    <!-- http://purl.obolibrary.org/obo/GAZ_00140820 -->

    <owl:NamedIndividual rdf:about="http://purl.obolibrary.org/obo/GAZ_00140820">
        <obo:RO_0001025 rdf:resource="http://purl.obolibrary.org/obo/GAZ_00140821"/>
        <obo:IAO_0000115>A piedmont glacier filling the N part of Moubray Bay, formed by the confluence of Moubray Glacier and ice streams falling from the W side of the S end of Adare Peninsula. The greater part of it is probably afloat.</obo:IAO_0000115>
        <oboInOwl:hasOBONamespace>GAZ</oboInOwl:hasOBONamespace>
        <oboInOwl:id>GAZ:00140820</oboInOwl:id>
        <rdfs:label>Moubray Piedmont Glacier</rdfs:label>
    </owl:NamedIndividual>
    


    <!-- http://purl.obolibrary.org/obo/GAZ_00140821 -->

    <owl:NamedIndividual rdf:about="http://purl.obolibrary.org/obo/GAZ_00140821">
        <obo:RO_0001025 rdf:resource="http://purl.obolibrary.org/obo/GAZ_00023304"/>
        <obo:IAO_0000115>A bay in western Ross Sea, indenting the coast of Victoria Land between Capes Roget and Hallett.</obo:IAO_0000115>
        <oboInOwl:hasOBONamespace>GAZ</oboInOwl:hasOBONamespace>
        <oboInOwl:id>GAZ:00140821</oboInOwl:id>
        <rdfs:label>Moubray Bay</rdfs:label>
    </owl:NamedIndividual>
    


    <!-- http://purl.obolibrary.org/obo/GAZ_00140825 -->

    <owl:NamedIndividual rdf:about="http://purl.obolibrary.org/obo/GAZ_00140825">
        <obo:RO_0001025 rdf:resource="http://purl.obolibrary.org/obo/GAZ_00014088"/>
        <obo:IAO_0000115>Heights which rise to 1,300 m (at Ravel Peak) east of Mozart Ice Piedmont in the north part of Alexander Island.</obo:IAO_0000115>
        <oboInOwl:hasOBONamespace>GAZ</oboInOwl:hasOBONamespace>
        <oboInOwl:id>GAZ:00140825</oboInOwl:id>
        <rdfs:label>Debussy Heights</rdfs:label>
    </owl:NamedIndividual>
    


    <!-- http://purl.obolibrary.org/obo/GAZ_00140826 -->

    <owl:NamedIndividual rdf:about="http://purl.obolibrary.org/obo/GAZ_00140826">
        <rdf:type rdf:resource="http://purl.obolibrary.org/obo/ENVO_00000032"/>
        <obo:RO_0001025 rdf:resource="http://purl.obolibrary.org/obo/GAZ_00004045"/>
        <obo:IAO_0000115>A gulf on the southeast side of the tip of Antarctic Peninsula, bordered on the northeast by the Joinville Island group and on the southwest by the James Ross Island group.</obo:IAO_0000115>
        <oboInOwl:hasOBONamespace>GAZ</oboInOwl:hasOBONamespace>
        <oboInOwl:id>GAZ:00140826</oboInOwl:id>
        <rdfs:label>Erebus and Terror Gulf</rdfs:label>
    </owl:NamedIndividual>
    


    <!-- http://purl.obolibrary.org/obo/GAZ_00140829 -->

    <owl:NamedIndividual rdf:about="http://purl.obolibrary.org/obo/GAZ_00140829">
        <obo:RO_0001025 rdf:resource="http://purl.obolibrary.org/obo/GAZ_00023304"/>
        <obo:IAO_0000115>A bank in the Ross Sea.</obo:IAO_0000115>
        <oboInOwl:hasOBONamespace>GAZ</oboInOwl:hasOBONamespace>
        <oboInOwl:id>GAZ:00140829</oboInOwl:id>
        <rdfs:label>Iselin Bank</rdfs:label>
    </owl:NamedIndividual>
    


    <!-- http://purl.obolibrary.org/obo/GAZ_00140830 -->

    <owl:NamedIndividual rdf:about="http://purl.obolibrary.org/obo/GAZ_00140830">
        <obo:RO_0001025 rdf:resource="http://purl.obolibrary.org/obo/GAZ_00141552"/>
        <obo:IAO_0000115>A marine bank with a least depth of 11 m in the southern approaches to Ryder Bay, Adelaide Island, 1.6 km south of Mikkelsen Islands.</obo:IAO_0000115>
        <oboInOwl:hasOBONamespace>GAZ</oboInOwl:hasOBONamespace>
        <oboInOwl:id>GAZ:00140830</oboInOwl:id>
        <rdfs:label>Ives Bank</rdfs:label>
    </owl:NamedIndividual>
    


    <!-- http://purl.obolibrary.org/obo/GAZ_00140832 -->

    <owl:NamedIndividual rdf:about="http://purl.obolibrary.org/obo/GAZ_00140832">
        <obo:RO_0001025 rdf:resource="http://purl.obolibrary.org/obo/GAZ_00023304"/>
        <obo:IAO_0000115>A northeast trending undersea basin of the central Ross continental shelf.</obo:IAO_0000115>
        <oboInOwl:hasOBONamespace>GAZ</oboInOwl:hasOBONamespace>
        <oboInOwl:id>GAZ:00140832</oboInOwl:id>
        <rdfs:label>JOIDES Basin</rdfs:label>
    </owl:NamedIndividual>
    


    <!-- http://purl.obolibrary.org/obo/GAZ_00140833 -->

    <owl:NamedIndividual rdf:about="http://purl.obolibrary.org/obo/GAZ_00140833">
        <obo:RO_0001025 rdf:resource="http://purl.obolibrary.org/obo/GAZ_00023304"/>
        <obo:IAO_0000115>An undersea basin named in association with the Nordenskjold Ice Tongue.</obo:IAO_0000115>
        <oboInOwl:hasOBONamespace>GAZ</oboInOwl:hasOBONamespace>
        <oboInOwl:id>GAZ:00140833</oboInOwl:id>
        <rdfs:label>Nordenskjold Basin</rdfs:label>
    </owl:NamedIndividual>
    


    <!-- http://purl.obolibrary.org/obo/GAZ_00140843 -->

    <owl:NamedIndividual rdf:about="http://purl.obolibrary.org/obo/GAZ_00140843">
        <obo:RO_0001025 rdf:resource="http://purl.obolibrary.org/obo/GAZ_00140059"/>
        <obo:IAO_0000115>An undersea trough north of the South Shetland Islands.</obo:IAO_0000115>
        <oboInOwl:hasOBONamespace>GAZ</oboInOwl:hasOBONamespace>
        <oboInOwl:id>GAZ:00140843</oboInOwl:id>
        <rdfs:label>South Shetland Trough</rdfs:label>
    </owl:NamedIndividual>
    


    <!-- http://purl.obolibrary.org/obo/GAZ_00140845 -->

    <owl:NamedIndividual rdf:about="http://purl.obolibrary.org/obo/GAZ_00140845">
        <rdf:type rdf:resource="http://purl.obolibrary.org/obo/ENVO_00000032"/>
        <obo:RO_0001025 rdf:resource="http://purl.obolibrary.org/obo/GAZ_00014085"/>
        <obo:IAO_0000115>An embayment about 115 miles wide along the coastline of Antarctica, lying seaward of the Getz Ice Shelf. Nearly a right angle in plan, its limits are described by Grant Island, Dean Island, and Siple Island, which are partially or wholly embedded in the ice shelf.</obo:IAO_0000115>
        <oboInOwl:hasOBONamespace>GAZ</oboInOwl:hasOBONamespace>
        <oboInOwl:id>GAZ:00140845</oboInOwl:id>
        <rdfs:label>Wrigley Gulf</rdfs:label>
    </owl:NamedIndividual>
    


    <!-- http://purl.obolibrary.org/obo/GAZ_00140870 -->

    <owl:NamedIndividual rdf:about="http://purl.obolibrary.org/obo/GAZ_00140870">
        <obo:RO_0001025 rdf:resource="http://purl.obolibrary.org/obo/GAZ_00051499"/>
        <obo:IAO_0000115>A bay lying at the junction of the western side of the Ninnis Glacier Tongue with the mainland.</obo:IAO_0000115>
        <oboInOwl:hasOBONamespace>GAZ</oboInOwl:hasOBONamespace>
        <oboInOwl:id>GAZ:00140870</oboInOwl:id>
        <rdfs:label>Doolette Bay</rdfs:label>
    </owl:NamedIndividual>
    


    <!-- http://purl.obolibrary.org/obo/GAZ_00140871 -->

    <owl:NamedIndividual rdf:about="http://purl.obolibrary.org/obo/GAZ_00140871">
        <obo:RO_0001025 rdf:resource="http://purl.obolibrary.org/obo/GAZ_00051499"/>
        <obo:IAO_0000115>A bay 7 mi wide between Penguin Point and Cape Bage.</obo:IAO_0000115>
        <oboInOwl:hasOBONamespace>GAZ</oboInOwl:hasOBONamespace>
        <oboInOwl:id>GAZ:00140871</oboInOwl:id>
        <rdfs:label>Murphy Bay</rdfs:label>
    </owl:NamedIndividual>
    


    <!-- http://purl.obolibrary.org/obo/GAZ_00140872 -->

    <owl:NamedIndividual rdf:about="http://purl.obolibrary.org/obo/GAZ_00140872">
        <obo:RO_0001025 rdf:resource="http://purl.obolibrary.org/obo/GAZ_00051499"/>
        <obo:IAO_0000115>An ice-filled recession of the coastline, 8 km wide, between Cape Bage and Cape Webb.</obo:IAO_0000115>
        <oboInOwl:hasOBONamespace>GAZ</oboInOwl:hasOBONamespace>
        <oboInOwl:id>GAZ:00140872</oboInOwl:id>
        <rdfs:label>Ainsworth Bay</rdfs:label>
    </owl:NamedIndividual>
    


    <!-- http://purl.obolibrary.org/obo/GAZ_00140873 -->

    <owl:NamedIndividual rdf:about="http://purl.obolibrary.org/obo/GAZ_00140873">
        <obo:RO_0001025 rdf:resource="http://purl.obolibrary.org/obo/GAZ_00141552"/>
        <obo:IAO_0000115>A bay 13 km wide, indenting the coast for 4.8 km between Cape Evensen and Cape Bellue, along the west coast of Graham Land.</obo:IAO_0000115>
        <oboInOwl:hasOBONamespace>GAZ</oboInOwl:hasOBONamespace>
        <oboInOwl:id>GAZ:00140873</oboInOwl:id>
        <rdfs:label>Auvert Bay</rdfs:label>
    </owl:NamedIndividual>
    


    <!-- http://purl.obolibrary.org/obo/GAZ_00140874 -->

    <owl:NamedIndividual rdf:about="http://purl.obolibrary.org/obo/GAZ_00140874">
        <obo:RO_0001025 rdf:resource="http://purl.obolibrary.org/obo/GAZ_00141552"/>
        <obo:IAO_0000115>A small bay lying 2.4 km southwest of D&apos;Ursel Point along the east side of Brabant Island, in the Palmer Archipelago.</obo:IAO_0000115>
        <oboInOwl:hasOBONamespace>GAZ</oboInOwl:hasOBONamespace>
        <oboInOwl:id>GAZ:00140874</oboInOwl:id>
        <rdfs:label>Avicenna Bay</rdfs:label>
    </owl:NamedIndividual>
    


    <!-- http://purl.obolibrary.org/obo/GAZ_00140875 -->

    <owl:NamedIndividual rdf:about="http://purl.obolibrary.org/obo/GAZ_00140875">
        <obo:RO_0001025 rdf:resource="http://purl.obolibrary.org/obo/GAZ_00014088"/>
        <obo:IAO_0000115>A deeply indented, ice-covered peninsula, 97 km long in a northeast-southwest direction and 97 km wide at its broadest part, forming the southwest part of Alexander Island, which lies off the southwestern portion of the Antarctic Peninsula. The Mendelssohn Inlet, the Brahms Inlet and the Verdi Inlet apparently intrude into it. The Bach Ice Shelf, Rossini Point and Berlioz Point are some distance away, on the Ronne Entrance from the Southern Ocean.</obo:IAO_0000115>
        <oboInOwl:hasOBONamespace>GAZ</oboInOwl:hasOBONamespace>
        <oboInOwl:id>GAZ:00140875</oboInOwl:id>
        <rdfs:label>Beethoven Peninsula</rdfs:label>
    </owl:NamedIndividual>
    


    <!-- http://purl.obolibrary.org/obo/GAZ_00140876 -->

    <owl:NamedIndividual rdf:about="http://purl.obolibrary.org/obo/GAZ_00140876">
        <obo:RO_0001025 rdf:resource="http://purl.obolibrary.org/obo/GAZ_00014084"/>
        <obo:IAO_0000115>An ice-filled inlet between Pesce Peninsula and Harris Peninsula, on the N side of Beethoven Peninsula, Alexander Island.</obo:IAO_0000115>
        <oboInOwl:hasOBONamespace>GAZ</oboInOwl:hasOBONamespace>
        <oboInOwl:id>GAZ:00140876</oboInOwl:id>
        <rdfs:label>Verdi Inlet</rdfs:label>
    </owl:NamedIndividual>
    


    <!-- http://purl.obolibrary.org/obo/GAZ_00140877 -->

    <owl:NamedIndividual rdf:about="http://purl.obolibrary.org/obo/GAZ_00140877">
        <obo:RO_0001025 rdf:resource="http://purl.obolibrary.org/obo/GAZ_00014084"/>
        <obo:IAO_0000115>An ice-filled inlet, 25 mi long and 9 mi wide, between Derocher peninsula and Eroica Peninsula on the N side of Beethoven Peninsula, Alexander Island.</obo:IAO_0000115>
        <oboInOwl:hasOBONamespace>GAZ</oboInOwl:hasOBONamespace>
        <oboInOwl:id>GAZ:00140877</oboInOwl:id>
        <rdfs:label>Mendelssohn Inlet</rdfs:label>
    </owl:NamedIndividual>
    


    <!-- http://purl.obolibrary.org/obo/GAZ_00140878 -->

    <owl:NamedIndividual rdf:about="http://purl.obolibrary.org/obo/GAZ_00140878">
        <obo:RO_0001025 rdf:resource="http://purl.obolibrary.org/obo/GAZ_00014084"/>
        <obo:IAO_0000115>An ice-filled inlet, 25 mi long and 6 mi wide, indenting the N side of Beethoven Peninsula on Alexander Island between Harris Peninsula and Derocher Peninsula.</obo:IAO_0000115>
        <oboInOwl:hasOBONamespace>GAZ</oboInOwl:hasOBONamespace>
        <oboInOwl:id>GAZ:00140878</oboInOwl:id>
        <rdfs:label>Brahms Inlet</rdfs:label>
    </owl:NamedIndividual>
    


    <!-- http://purl.obolibrary.org/obo/GAZ_00140879 -->

    <owl:NamedIndividual rdf:about="http://purl.obolibrary.org/obo/GAZ_00140879">
        <obo:RO_0001025 rdf:resource="http://purl.obolibrary.org/obo/GAZ_00140875"/>
        <obo:IAO_0000115>A broad snow-covered peninsula surmounted by Mount Lee, between Verdi Inlet and Brahms Inlet on the N side of Beethoven Peninsula, Alexander Island.</obo:IAO_0000115>
        <oboInOwl:hasOBONamespace>GAZ</oboInOwl:hasOBONamespace>
        <oboInOwl:id>GAZ:00140879</oboInOwl:id>
        <rdfs:label>Harris Peninsula</rdfs:label>
    </owl:NamedIndividual>
    


    <!-- http://purl.obolibrary.org/obo/GAZ_00140880 -->

    <owl:NamedIndividual rdf:about="http://purl.obolibrary.org/obo/GAZ_00140880">
        <obo:RO_0001025 rdf:resource="http://purl.obolibrary.org/obo/GAZ_00014088"/>
        <obo:IAO_0000115>An ice-covered peninsula lying N of Beethoven Peninsula and Mendelssohn Inlet in W Alexander Island.</obo:IAO_0000115>
        <oboInOwl:hasOBONamespace>GAZ</oboInOwl:hasOBONamespace>
        <oboInOwl:id>GAZ:00140880</oboInOwl:id>
        <rdfs:label>Eroica Peninsula</rdfs:label>
    </owl:NamedIndividual>
    


    <!-- http://purl.obolibrary.org/obo/GAZ_00140881 -->

    <owl:NamedIndividual rdf:about="http://purl.obolibrary.org/obo/GAZ_00140881">
        <obo:RO_0001025 rdf:resource="http://purl.obolibrary.org/obo/GAZ_00014088"/>
        <obo:IAO_0000115>A snow-covered peninsula between Brahms Inlet and Mendelssohn Inlet on the N side of Beethoven Peninsula, Alexander Island.</obo:IAO_0000115>
        <oboInOwl:hasOBONamespace>GAZ</oboInOwl:hasOBONamespace>
        <oboInOwl:id>GAZ:00140881</oboInOwl:id>
        <rdfs:label>Derocher Peninsula</rdfs:label>
    </owl:NamedIndividual>
    


    <!-- http://purl.obolibrary.org/obo/GAZ_00140885 -->

    <owl:NamedIndividual rdf:about="http://purl.obolibrary.org/obo/GAZ_00140885">
        <obo:RO_0001025 rdf:resource="http://purl.obolibrary.org/obo/GAZ_00140310"/>
        <obo:IAO_0000115>A group of rocky, irregular islands which extends about 11 mi in an E-W direction, lying in the S part of the entrance to Edward VlII Bay.</obo:IAO_0000115>
        <oboInOwl:hasOBONamespace>GAZ</oboInOwl:hasOBONamespace>
        <oboInOwl:id>GAZ:00140885</oboInOwl:id>
        <rdfs:label>Oygarden Group</rdfs:label>
    </owl:NamedIndividual>
    


    <!-- http://purl.obolibrary.org/obo/GAZ_00140887 -->

    <owl:NamedIndividual rdf:about="http://purl.obolibrary.org/obo/GAZ_00140887">
        <obo:RO_0001025 rdf:resource="http://purl.obolibrary.org/obo/GAZ_00014088"/>
        <obo:IAO_0000115>A distinctive ice-cliffed cape at the southwest end of Adelaide Island, 16 km northwest of Avian Island.</obo:IAO_0000115>
        <oboInOwl:hasOBONamespace>GAZ</oboInOwl:hasOBONamespace>
        <oboInOwl:id>GAZ:00140887</oboInOwl:id>
        <rdfs:label>Cape Adriasola</rdfs:label>
    </owl:NamedIndividual>
    


    <!-- http://purl.obolibrary.org/obo/GAZ_00140891 -->

    <owl:NamedIndividual rdf:about="http://purl.obolibrary.org/obo/GAZ_00140891">
        <obo:RO_0001025 rdf:resource="http://purl.obolibrary.org/obo/GAZ_00045055"/>
        <obo:IAO_0000115>A bold, dark-colored bluff marking the north end of Wiencke Island, in the Palmer Archipelago.</obo:IAO_0000115>
        <oboInOwl:hasOBONamespace>GAZ</oboInOwl:hasOBONamespace>
        <oboInOwl:id>GAZ:00140891</oboInOwl:id>
        <rdfs:label>Cape Astrup</rdfs:label>
    </owl:NamedIndividual>
    


    <!-- http://purl.obolibrary.org/obo/GAZ_00140893 -->

    <owl:NamedIndividual rdf:about="http://purl.obolibrary.org/obo/GAZ_00140893">
        <obo:RO_0001025 rdf:resource="http://purl.obolibrary.org/obo/GAZ_00004045"/>
        <obo:IAO_0000115>A Large pouch-shaped, ice-filled embayment between Cape Kidson and Cape Brooks, along the E coast of Palmer Land.</obo:IAO_0000115>
        <oboInOwl:hasOBONamespace>GAZ</oboInOwl:hasOBONamespace>
        <oboInOwl:id>GAZ:00140893</oboInOwl:id>
        <rdfs:label>New Bedford Inlet</rdfs:label>
    </owl:NamedIndividual>
    


    <!-- http://purl.obolibrary.org/obo/GAZ_00140895 -->

    <owl:NamedIndividual rdf:about="http://purl.obolibrary.org/obo/GAZ_00140895">
        <obo:RO_0001025 rdf:resource="http://purl.obolibrary.org/obo/GAZ_00014085"/>
        <obo:IAO_0000115>A bay about 20 mi long and wide, lying S of Canisteo Peninsula at the E end of Amundsen Sea. The S limit of the bay is formed by the Backer Islands and an ice shelf which separates this bay from Pine Island Bay.</obo:IAO_0000115>
        <oboInOwl:hasOBONamespace>GAZ</oboInOwl:hasOBONamespace>
        <oboInOwl:id>GAZ:00140895</oboInOwl:id>
        <rdfs:label>Cranton Bay</rdfs:label>
    </owl:NamedIndividual>
    


    <!-- http://purl.obolibrary.org/obo/GAZ_00140896 -->

    <owl:NamedIndividual rdf:about="http://purl.obolibrary.org/obo/GAZ_00140896">
        <obo:RO_0001025 rdf:resource="http://purl.obolibrary.org/obo/GAZ_00140895"/>
        <obo:IAO_0000115>A chain of small islands at the S side of Cranton Bay. The islands trend NW for 12 mi from the ice shelf which forms the S limit of the bay.</obo:IAO_0000115>
        <oboInOwl:hasOBONamespace>GAZ</oboInOwl:hasOBONamespace>
        <oboInOwl:id>GAZ:00140896</oboInOwl:id>
        <rdfs:label>Backer Islands</rdfs:label>
    </owl:NamedIndividual>
    


    <!-- http://purl.obolibrary.org/obo/GAZ_00140897 -->

    <owl:NamedIndividual rdf:about="http://purl.obolibrary.org/obo/GAZ_00140897">
        <obo:RO_0001025 rdf:resource="http://purl.obolibrary.org/obo/GAZ_00014085"/>
        <obo:IAO_0000115>A body of water about 15 mi wide, lying immediately W of Cosgrove Ice Shelf and occupying the outer (west) part of the embayment between King and Canisteo Peninsulas.</obo:IAO_0000115>
        <oboInOwl:hasOBONamespace>GAZ</oboInOwl:hasOBONamespace>
        <oboInOwl:id>GAZ:00140897</oboInOwl:id>
        <rdfs:label>Ferrero Bay</rdfs:label>
    </owl:NamedIndividual>
    


    <!-- http://purl.obolibrary.org/obo/GAZ_00140900 -->

    <owl:NamedIndividual rdf:about="http://purl.obolibrary.org/obo/GAZ_00140900">
        <obo:RO_0001025 rdf:resource="http://purl.obolibrary.org/obo/GAZ_00140310"/>
        <obo:IAO_0000115>Three small islands 15 mi SW of Austnes Point in the W part of Edward VIII Bay.</obo:IAO_0000115>
        <oboInOwl:hasOBONamespace>GAZ</oboInOwl:hasOBONamespace>
        <oboInOwl:id>GAZ:00140900</oboInOwl:id>
        <rdfs:label>Patricia Islands</rdfs:label>
    </owl:NamedIndividual>
    


    <!-- http://purl.obolibrary.org/obo/GAZ_00140901 -->

    <owl:NamedIndividual rdf:about="http://purl.obolibrary.org/obo/GAZ_00140901">
        <obo:RO_0001025 rdf:resource="http://purl.obolibrary.org/obo/GAZ_00004381"/>
        <obo:IAO_0000115>A rocky point immediately southeast of Biscoe Point and 3.2 km northwest of Cape Lancaster on the south side of Anvers Island, in the Palmer Archipelago.</obo:IAO_0000115>
        <oboInOwl:hasOBONamespace>GAZ</oboInOwl:hasOBONamespace>
        <oboInOwl:id>GAZ:00140901</oboInOwl:id>
        <rdfs:label>Access Point</rdfs:label>
    </owl:NamedIndividual>
    


    <!-- http://purl.obolibrary.org/obo/GAZ_00140902 -->

    <owl:NamedIndividual rdf:about="http://purl.obolibrary.org/obo/GAZ_00140902">
        <obo:RO_0001025 rdf:resource="http://purl.obolibrary.org/obo/GAZ_00023358"/>
        <obo:IAO_0000115>An ice-covered point 1.6 km southeast of Cone Hill on the east side of Hut Point Peninsula, Ross Island.</obo:IAO_0000115>
        <oboInOwl:hasOBONamespace>GAZ</oboInOwl:hasOBONamespace>
        <oboInOwl:id>GAZ:00140902</oboInOwl:id>
        <rdfs:label>Ackley Point</rdfs:label>
    </owl:NamedIndividual>
    


    <!-- http://purl.obolibrary.org/obo/GAZ_00140904 -->

    <owl:NamedIndividual rdf:about="http://purl.obolibrary.org/obo/GAZ_00140904">
        <obo:RO_0001025 rdf:resource="http://purl.obolibrary.org/obo/GAZ_00141552"/>
        <obo:IAO_0000115>A Bay 3 mi long, lying between Cape Renard and Aguda Point on the W coast of Graham Land.</obo:IAO_0000115>
        <oboInOwl:hasOBONamespace>GAZ</oboInOwl:hasOBONamespace>
        <oboInOwl:id>GAZ:00140904</oboInOwl:id>
        <rdfs:label>Hidden Bay</rdfs:label>
    </owl:NamedIndividual>
    


    <!-- http://purl.obolibrary.org/obo/GAZ_00140907 -->

    <owl:NamedIndividual rdf:about="http://purl.obolibrary.org/obo/GAZ_00140907">
        <obo:RO_0001025 rdf:resource="http://purl.obolibrary.org/obo/GAZ_00139595"/>
        <obo:IAO_0000115>An exposed rocky point on the southwest side of Bransfield Island in Antarctic Sound.</obo:IAO_0000115>
        <oboInOwl:hasOBONamespace>GAZ</oboInOwl:hasOBONamespace>
        <oboInOwl:id>GAZ:00140907</oboInOwl:id>
        <rdfs:label>Archibald Point</rdfs:label>
    </owl:NamedIndividual>
    


    <!-- http://purl.obolibrary.org/obo/GAZ_00140911 -->

    <owl:NamedIndividual rdf:about="http://purl.obolibrary.org/obo/GAZ_00140911">
        <obo:RO_0001025 rdf:resource="http://purl.obolibrary.org/obo/GAZ_00023294"/>
        <obo:IAO_0000115>A bay indenting the SW shore of Lutzow-Holm Bay immediately W of Botnneset Peninsula.</obo:IAO_0000115>
        <oboInOwl:hasOBONamespace>GAZ</oboInOwl:hasOBONamespace>
        <oboInOwl:id>GAZ:00140911</oboInOwl:id>
        <rdfs:label>Fletta Bay</rdfs:label>
    </owl:NamedIndividual>
    


    <!-- http://purl.obolibrary.org/obo/GAZ_00140912 -->

    <owl:NamedIndividual rdf:about="http://purl.obolibrary.org/obo/GAZ_00140912">
        <obo:RO_0001025 rdf:resource="http://purl.obolibrary.org/obo/GAZ_00023294"/>
        <obo:IAO_0000115>A bay between Botnneset and Djupvikneset Peninsulas in the SW part of Lutzow-Holm Bay.</obo:IAO_0000115>
        <oboInOwl:hasOBONamespace>GAZ</oboInOwl:hasOBONamespace>
        <oboInOwl:id>GAZ:00140912</oboInOwl:id>
        <rdfs:label>Djupvika</rdfs:label>
    </owl:NamedIndividual>
    


    <!-- http://purl.obolibrary.org/obo/GAZ_00140914 -->

    <owl:NamedIndividual rdf:about="http://purl.obolibrary.org/obo/GAZ_00140914">
        <obo:RO_0001025 rdf:resource="http://purl.obolibrary.org/obo/GAZ_00023294"/>
        <obo:IAO_0000115>An island lying near the W side of the entrance to Havsbotn in Lutzow-Holm Bay.</obo:IAO_0000115>
        <oboInOwl:hasOBONamespace>GAZ</oboInOwl:hasOBONamespace>
        <oboInOwl:id>GAZ:00140914</oboInOwl:id>
        <rdfs:label>Padda</rdfs:label>
    </owl:NamedIndividual>
    


    <!-- http://purl.obolibrary.org/obo/GAZ_00140915 -->

    <owl:NamedIndividual rdf:about="http://purl.obolibrary.org/obo/GAZ_00140915">
        <rdf:type rdf:resource="http://purl.obolibrary.org/obo/ENVO_00000305"/>
        <obo:RO_0001025 rdf:resource="http://purl.obolibrary.org/obo/GAZ_00140914"/>
        <obo:IAO_0000115>A headland forming the northeast extremity of Padda Island in Lutzow-Holm Bay.</obo:IAO_0000115>
        <oboInOwl:hasOBONamespace>GAZ</oboInOwl:hasOBONamespace>
        <oboInOwl:id>GAZ:00140915</oboInOwl:id>
        <rdfs:label>Austpynten</rdfs:label>
    </owl:NamedIndividual>
    


    <!-- http://purl.obolibrary.org/obo/GAZ_00140916 -->

    <owl:NamedIndividual rdf:about="http://purl.obolibrary.org/obo/GAZ_00140916">
        <rdf:type rdf:resource="http://purl.obolibrary.org/obo/ENVO_00000305"/>
        <obo:RO_0001025 rdf:resource="http://purl.obolibrary.org/obo/GAZ_00045105"/>
        <obo:IAO_0000115>A headland 6 km northeast of Borge Point on the east side of Trinity Island, in the Palmer Archipelago.</obo:IAO_0000115>
        <oboInOwl:hasOBONamespace>GAZ</oboInOwl:hasOBONamespace>
        <oboInOwl:id>GAZ:00140916</oboInOwl:id>
        <rdfs:label>Awl Point</rdfs:label>
    </owl:NamedIndividual>
    


    <!-- http://purl.obolibrary.org/obo/GAZ_00140917 -->

    <owl:NamedIndividual rdf:about="http://purl.obolibrary.org/obo/GAZ_00140917">
        <rdf:type rdf:resource="http://purl.obolibrary.org/obo/ENVO_00000305"/>
        <obo:RO_0001025 rdf:resource="http://purl.obolibrary.org/obo/GAZ_00045105"/>
        <obo:IAO_0000115>A headland forming the E side of Mikkelsen Harbor, Trinity Island, in the Palmer Archipelago.</obo:IAO_0000115>
        <oboInOwl:hasOBONamespace>GAZ</oboInOwl:hasOBONamespace>
        <oboInOwl:id>GAZ:00140917</oboInOwl:id>
        <rdfs:label>Borge Point</rdfs:label>
    </owl:NamedIndividual>
    


    <!-- http://purl.obolibrary.org/obo/GAZ_00140925 -->

    <owl:NamedIndividual rdf:about="http://purl.obolibrary.org/obo/GAZ_00140925">
        <obo:RO_0001025 rdf:resource="http://purl.obolibrary.org/obo/GAZ_00011782"/>
        <obo:IAO_0000115>A narrow island lying 2 mi N of Inexpressible Island and just W of the Northern Foothills, along the coast of Victoria Land.</obo:IAO_0000115>
        <oboInOwl:hasOBONamespace>GAZ</oboInOwl:hasOBONamespace>
        <oboInOwl:id>GAZ:00140925</oboInOwl:id>
        <rdfs:label>Vegetation Island</rdfs:label>
    </owl:NamedIndividual>
    


    <!-- http://purl.obolibrary.org/obo/GAZ_00140927 -->

    <owl:NamedIndividual rdf:about="http://purl.obolibrary.org/obo/GAZ_00140927">
        <rdf:type rdf:resource="http://purl.obolibrary.org/obo/ENVO_00000305"/>
        <obo:RO_0001025 rdf:resource="http://purl.obolibrary.org/obo/GAZ_00045044"/>
        <obo:IAO_0000115>A cape at the foot of Mount Siple on the north coast of Siple Island, just southward of Lauff Island.</obo:IAO_0000115>
        <oboInOwl:hasOBONamespace>GAZ</oboInOwl:hasOBONamespace>
        <oboInOwl:id>GAZ:00140927</oboInOwl:id>
        <rdfs:label>Cape Dart</rdfs:label>
    </owl:NamedIndividual>
    


    <!-- http://purl.obolibrary.org/obo/GAZ_00140928 -->

    <owl:NamedIndividual rdf:about="http://purl.obolibrary.org/obo/GAZ_00140928">
        <obo:RO_0001025 rdf:resource="http://purl.obolibrary.org/obo/GAZ_00014085"/>
        <obo:IAO_0000115>A small island lying 2 mi north of Cape Dart, Siple Island, off the coast of Marie Byrd Land.</obo:IAO_0000115>
        <oboInOwl:hasOBONamespace>GAZ</oboInOwl:hasOBONamespace>
        <oboInOwl:id>GAZ:00140928</oboInOwl:id>
        <rdfs:label>Lauff Island</rdfs:label>
    </owl:NamedIndividual>
    


    <!-- http://purl.obolibrary.org/obo/GAZ_00140931 -->

    <owl:NamedIndividual rdf:about="http://purl.obolibrary.org/obo/GAZ_00140931">
        <obo:RO_0001025 rdf:resource="http://purl.obolibrary.org/obo/GAZ_00004045"/>
        <obo:IAO_0000115>A large ice-filled inlet, 26 km wide at its entrance between Foyn Point and Cape Disappointment, on the east coast of Graham Land.</obo:IAO_0000115>
        <oboInOwl:hasOBONamespace>GAZ</oboInOwl:hasOBONamespace>
        <oboInOwl:id>GAZ:00140931</oboInOwl:id>
        <rdfs:label>Exasperation Inlet</rdfs:label>
    </owl:NamedIndividual>
    


    <!-- http://purl.obolibrary.org/obo/GAZ_00140933 -->

    <owl:NamedIndividual rdf:about="http://purl.obolibrary.org/obo/GAZ_00140933">
        <obo:RO_0001025 rdf:resource="http://purl.obolibrary.org/obo/GAZ_00051133"/>
        <obo:IAO_0000115>An area of the Larsen Ice Shelf immediately NW of Jason Peninsula. It is bounded by Tashtego Point and Chapman Point.</obo:IAO_0000115>
        <oboInOwl:hasOBONamespace>GAZ</oboInOwl:hasOBONamespace>
        <oboInOwl:id>GAZ:00140933</oboInOwl:id>
        <rdfs:label>Scar Inlet</rdfs:label>
    </owl:NamedIndividual>
    


    <!-- http://purl.obolibrary.org/obo/GAZ_00140943 -->

    <owl:NamedIndividual rdf:about="http://purl.obolibrary.org/obo/GAZ_00140943">
        <obo:RO_0001025 rdf:resource="http://purl.obolibrary.org/obo/GAZ_00014140"/>
        <obo:IAO_0000115>An ice-covered cape which forms the west extremity of Thurston Island.</obo:IAO_0000115>
        <oboInOwl:hasOBONamespace>GAZ</oboInOwl:hasOBONamespace>
        <oboInOwl:id>GAZ:00140943</oboInOwl:id>
        <rdfs:label>Cape Flying Fish</rdfs:label>
    </owl:NamedIndividual>
    


    <!-- http://purl.obolibrary.org/obo/GAZ_00140950 -->

    <owl:NamedIndividual rdf:about="http://purl.obolibrary.org/obo/GAZ_00140950">
        <obo:RO_0001025 rdf:resource="http://purl.obolibrary.org/obo/GAZ_00017744"/>
        <obo:IAO_0000115>The southeast point of Low Island, in the South Shetland Islands.</obo:IAO_0000115>
        <oboInOwl:hasOBONamespace>GAZ</oboInOwl:hasOBONamespace>
        <oboInOwl:id>GAZ:00140950</oboInOwl:id>
        <rdfs:label>Cape Hooker</rdfs:label>
    </owl:NamedIndividual>
    


    <!-- http://purl.obolibrary.org/obo/GAZ_00140952 -->

    <owl:NamedIndividual rdf:about="http://purl.obolibrary.org/obo/GAZ_00140952">
        <obo:RO_0001025 rdf:resource="http://purl.obolibrary.org/obo/GAZ_00004381"/>
        <obo:IAO_0000115>A prominent point 13 km west-southwest of Ryswyck Point, on the east side of Anvers Island, in the Palmer Archipelago.</obo:IAO_0000115>
        <oboInOwl:hasOBONamespace>GAZ</oboInOwl:hasOBONamespace>
        <oboInOwl:id>GAZ:00140952</oboInOwl:id>
        <rdfs:label>Iceberg Point</rdfs:label>
    </owl:NamedIndividual>
    


    <!-- http://purl.obolibrary.org/obo/GAZ_00140953 -->

    <owl:NamedIndividual rdf:about="http://purl.obolibrary.org/obo/GAZ_00140953">
        <rdf:type rdf:resource="http://purl.obolibrary.org/obo/ENVO_00000305"/>
        <obo:RO_0001025 rdf:resource="http://purl.obolibrary.org/obo/GAZ_00004381"/>
        <obo:IAO_0000115>A headland marking the east extremity of Anvers Island, in the Palmer Archipelago.</obo:IAO_0000115>
        <oboInOwl:hasOBONamespace>GAZ</oboInOwl:hasOBONamespace>
        <oboInOwl:id>GAZ:00140953</oboInOwl:id>
        <rdfs:label>Ryswyck Point</rdfs:label>
    </owl:NamedIndividual>
    


    <!-- http://purl.obolibrary.org/obo/GAZ_00140956 -->

    <owl:NamedIndividual rdf:about="http://purl.obolibrary.org/obo/GAZ_00140956">
        <rdf:type rdf:resource="http://purl.obolibrary.org/obo/ENVO_00000305"/>
        <obo:RO_0001025 rdf:resource="http://purl.obolibrary.org/obo/GAZ_00014120"/>
        <obo:IAO_0000115>A headland on the northwest side of Harmony Cove, Nelson Island, in the South Shetland Islands.</obo:IAO_0000115>
        <oboInOwl:hasOBONamespace>GAZ</oboInOwl:hasOBONamespace>
        <oboInOwl:id>GAZ:00140956</oboInOwl:id>
        <rdfs:label>Inca Point</rdfs:label>
    </owl:NamedIndividual>
    


    <!-- http://purl.obolibrary.org/obo/GAZ_00140957 -->

    <owl:NamedIndividual rdf:about="http://purl.obolibrary.org/obo/GAZ_00140957">
        <obo:RO_0001025 rdf:resource="http://purl.obolibrary.org/obo/GAZ_00140059"/>
        <obo:IAO_0000115>A cove entered between Harmony Point and The Toe on the W side of Nelson Island, in the South Shetland Islands.</obo:IAO_0000115>
        <oboInOwl:hasOBONamespace>GAZ</oboInOwl:hasOBONamespace>
        <oboInOwl:id>GAZ:00140957</oboInOwl:id>
        <rdfs:label>Harmony Cove</rdfs:label>
    </owl:NamedIndividual>
    


    <!-- http://purl.obolibrary.org/obo/GAZ_00140959 -->

    <owl:NamedIndividual rdf:about="http://purl.obolibrary.org/obo/GAZ_00140959">
        <obo:RO_0001025 rdf:resource="http://purl.obolibrary.org/obo/GAZ_00139892"/>
        <obo:IAO_0000115>An ice-covered island 2 mi long, lying 1.5 mi E of Index Point, Victoria Land, in the N part of Lady Newnes Bay. The feature appears to be barely emerging above the ice at the terminus of Mariner Glacier.</obo:IAO_0000115>
        <oboInOwl:hasOBONamespace>GAZ</oboInOwl:hasOBONamespace>
        <oboInOwl:id>GAZ:00140959</oboInOwl:id>
        <rdfs:label>Emerging Island</rdfs:label>
    </owl:NamedIndividual>
    


    <!-- http://purl.obolibrary.org/obo/GAZ_00140960 -->

    <owl:NamedIndividual rdf:about="http://purl.obolibrary.org/obo/GAZ_00140960">
        <obo:RO_0001025 rdf:resource="http://purl.obolibrary.org/obo/GAZ_00005837"/>
        <obo:IAO_0000115>A dark rock promontory separating Norvegia Bay and Sandefjord Cove on the west side of Peter I Island.</obo:IAO_0000115>
        <oboInOwl:hasOBONamespace>GAZ</oboInOwl:hasOBONamespace>
        <oboInOwl:id>GAZ:00140960</oboInOwl:id>
        <rdfs:label>Cape Ingrid</rdfs:label>
    </owl:NamedIndividual>
    


    <!-- http://purl.obolibrary.org/obo/GAZ_00140961 -->

    <owl:NamedIndividual rdf:about="http://purl.obolibrary.org/obo/GAZ_00140961">
        <obo:RO_0001025 rdf:resource="http://purl.obolibrary.org/obo/GAZ_00014084"/>
        <obo:IAO_0000115>A cove between Cape Ingrid and the terminus of Tofte Glacier on the west side of Peter I Island.</obo:IAO_0000115>
        <oboInOwl:hasOBONamespace>GAZ</oboInOwl:hasOBONamespace>
        <oboInOwl:id>GAZ:00140961</oboInOwl:id>
        <rdfs:label>Sandefjord Cove</rdfs:label>
    </owl:NamedIndividual>
    


    <!-- http://purl.obolibrary.org/obo/GAZ_00140962 -->

    <owl:NamedIndividual rdf:about="http://purl.obolibrary.org/obo/GAZ_00140962">
        <obo:RO_0001025 rdf:resource="http://purl.obolibrary.org/obo/GAZ_00014084"/>
        <obo:IAO_0000115>A cove at the north side of Cape Ingrid on the west side of Peter I Island.</obo:IAO_0000115>
        <oboInOwl:hasOBONamespace>GAZ</oboInOwl:hasOBONamespace>
        <oboInOwl:id>GAZ:00140962</oboInOwl:id>
        <rdfs:label>Norvegia Bay</rdfs:label>
    </owl:NamedIndividual>
    


    <!-- http://purl.obolibrary.org/obo/GAZ_00140963 -->

    <owl:NamedIndividual rdf:about="http://purl.obolibrary.org/obo/GAZ_00140963">
        <obo:RO_0001025 rdf:resource="http://purl.obolibrary.org/obo/GAZ_00005837"/>
        <obo:IAO_0000115>A glacier immediately south of Sandefjord Cove on the west side of Peter I Island.</obo:IAO_0000115>
        <oboInOwl:hasOBONamespace>GAZ</oboInOwl:hasOBONamespace>
        <oboInOwl:id>GAZ:00140963</oboInOwl:id>
        <rdfs:label>Tofte Glacier</rdfs:label>
    </owl:NamedIndividual>
    


    <!-- http://purl.obolibrary.org/obo/GAZ_00140965 -->

    <owl:NamedIndividual rdf:about="http://purl.obolibrary.org/obo/GAZ_00140965">
        <obo:RO_0001025 rdf:resource="http://purl.obolibrary.org/obo/GAZ_00014100"/>
        <obo:IAO_0000115>A small volcanic peak projecting through the ice sheet covering the southeast extremity of White Island, in the Ross Archipelago.</obo:IAO_0000115>
        <oboInOwl:hasOBONamespace>GAZ</oboInOwl:hasOBONamespace>
        <oboInOwl:id>GAZ:00140965</oboInOwl:id>
        <rdfs:label>Isolation Point</rdfs:label>
    </owl:NamedIndividual>
    


    <!-- http://purl.obolibrary.org/obo/GAZ_00140969 -->

    <owl:NamedIndividual rdf:about="http://purl.obolibrary.org/obo/GAZ_00140969">
        <obo:RO_0001025 rdf:resource="http://purl.obolibrary.org/obo/GAZ_00004045"/>
        <obo:IAO_0000115>A bay, 4.0 km wide at its mouth and extending 4.8 km inland, lying north of Jade Point, Trinity Peninsula.</obo:IAO_0000115>
        <oboInOwl:hasOBONamespace>GAZ</oboInOwl:hasOBONamespace>
        <oboInOwl:id>GAZ:00140969</oboInOwl:id>
        <rdfs:label>Eyrie Bay</rdfs:label>
    </owl:NamedIndividual>
    


    <!-- http://purl.obolibrary.org/obo/GAZ_00140974 -->

    <owl:NamedIndividual rdf:about="http://purl.obolibrary.org/obo/GAZ_00140974">
        <obo:RO_0001025 rdf:resource="http://purl.obolibrary.org/obo/GAZ_00014084"/>
        <obo:IAO_0000115>An ice-filled inlet which recedes 15 mi SW between Cape Mackintosh and the coastline south of Cape Herdman, along the E coast of Palmer Land.</obo:IAO_0000115>
        <oboInOwl:hasOBONamespace>GAZ</oboInOwl:hasOBONamespace>
        <oboInOwl:id>GAZ:00140974</oboInOwl:id>
        <rdfs:label>Mason Inlet</rdfs:label>
    </owl:NamedIndividual>
    


    <!-- http://purl.obolibrary.org/obo/GAZ_00140975 -->

    <owl:NamedIndividual rdf:about="http://purl.obolibrary.org/obo/GAZ_00140975">
        <obo:RO_0001025 rdf:resource="http://purl.obolibrary.org/obo/GAZ_00014084"/>
        <obo:IAO_0000115>A narrow ice-filled inlet which recedes N 10 mi between Cape Kidson and the SW end of Kemp Peninsula, along the E coast of Palmer Land.</obo:IAO_0000115>
        <oboInOwl:hasOBONamespace>GAZ</oboInOwl:hasOBONamespace>
        <oboInOwl:id>GAZ:00140975</oboInOwl:id>
        <rdfs:label>Mossman Inlet</rdfs:label>
    </owl:NamedIndividual>
    


    <!-- http://purl.obolibrary.org/obo/GAZ_00140978 -->

    <owl:NamedIndividual rdf:about="http://purl.obolibrary.org/obo/GAZ_00140978">
        <obo:RO_0001025 rdf:resource="http://purl.obolibrary.org/obo/GAZ_00014084"/>
        <obo:IAO_0000115>An ice-filled inlet, 12 mi wide, which recedes about 22 mi W from its entrance between Capes Darlington and Knowles, along the E coast of Palmer Land.</obo:IAO_0000115>
        <oboInOwl:hasOBONamespace>GAZ</oboInOwl:hasOBONamespace>
        <oboInOwl:id>GAZ:00140978</oboInOwl:id>
        <rdfs:label>Hilton Inlet</rdfs:label>
    </owl:NamedIndividual>
    


    <!-- http://purl.obolibrary.org/obo/GAZ_00140980 -->

    <owl:NamedIndividual rdf:about="http://purl.obolibrary.org/obo/GAZ_00140980">
        <obo:RO_0001025 rdf:resource="http://purl.obolibrary.org/obo/GAZ_00023304"/>
        <obo:IAO_0000115>A seamount.</obo:IAO_0000115>
        <oboInOwl:hasOBONamespace>GAZ</oboInOwl:hasOBONamespace>
        <oboInOwl:id>GAZ:00140980</oboInOwl:id>
        <rdfs:label>Iselin Seamount</rdfs:label>
    </owl:NamedIndividual>
    


    <!-- http://purl.obolibrary.org/obo/GAZ_00140981 -->

    <owl:NamedIndividual rdf:about="http://purl.obolibrary.org/obo/GAZ_00140981">
        <obo:RO_0001025 rdf:resource="http://purl.obolibrary.org/obo/GAZ_00023304"/>
        <obo:IAO_0000115>A bank.</obo:IAO_0000115>
        <oboInOwl:hasOBONamespace>GAZ</oboInOwl:hasOBONamespace>
        <oboInOwl:id>GAZ:00140981</oboInOwl:id>
        <rdfs:label>Shirase Bank</rdfs:label>
    </owl:NamedIndividual>
    


    <!-- http://purl.obolibrary.org/obo/GAZ_00140982 -->

    <owl:NamedIndividual rdf:about="http://purl.obolibrary.org/obo/GAZ_00140982">
        <rdf:type rdf:resource="http://purl.obolibrary.org/obo/ENVO_00000032"/>
        <obo:RO_0001025 rdf:resource="http://purl.obolibrary.org/obo/GAZ_00051500"/>
        <obo:IAO_0000115>A bight in the western part of the coast of Enderby Land.</obo:IAO_0000115>
        <oboInOwl:hasOBONamespace>GAZ</oboInOwl:hasOBONamespace>
        <oboInOwl:id>GAZ:00140982</oboInOwl:id>
        <rdfs:label>Alasheyev Bight</rdfs:label>
    </owl:NamedIndividual>
    


    <!-- http://purl.obolibrary.org/obo/GAZ_00140983 -->

    <owl:NamedIndividual rdf:about="http://purl.obolibrary.org/obo/GAZ_00140983">
        <obo:RO_0001025 rdf:resource="http://purl.obolibrary.org/obo/GAZ_00004045"/>
        <obo:IAO_0000115>An ice-filled inlet 5 to 10 mi wide, which recedes W 14 mi between Rock Pile Peaks and Joerg Peninsula, on the E coast of Graham Land.</obo:IAO_0000115>
        <oboInOwl:hasOBONamespace>GAZ</oboInOwl:hasOBONamespace>
        <oboInOwl:id>GAZ:00140983</oboInOwl:id>
        <rdfs:label>Solberg Inlet</rdfs:label>
    </owl:NamedIndividual>
    


    <!-- http://purl.obolibrary.org/obo/GAZ_00140984 -->

    <owl:NamedIndividual rdf:about="http://purl.obolibrary.org/obo/GAZ_00140984">
        <rdf:type rdf:resource="http://purl.obolibrary.org/obo/ENVO_00000220"/>
        <obo:RO_0001025 rdf:resource="http://purl.obolibrary.org/obo/GAZ_00051499"/>
        <obo:IAO_0000115>A small island group off the Budd Coast of Wilkes Land in Australian Antarctica.</obo:IAO_0000115>
        <oboInOwl:hasOBONamespace>GAZ</oboInOwl:hasOBONamespace>
        <oboInOwl:id>GAZ:00140984</oboInOwl:id>
        <rdfs:label>Hatch Islands</rdfs:label>
    </owl:NamedIndividual>
    


    <!-- http://purl.obolibrary.org/obo/GAZ_00140988 -->

    <owl:NamedIndividual rdf:about="http://purl.obolibrary.org/obo/GAZ_00140988">
        <obo:RO_0001025 rdf:resource="http://purl.obolibrary.org/obo/GAZ_00023304"/>
        <obo:IAO_0000115>A bay 1.6 km wide, lying just southeast of Discovery Bluff in Granite Harbor, Victoria Land.</obo:IAO_0000115>
        <oboInOwl:hasOBONamespace>GAZ</oboInOwl:hasOBONamespace>
        <oboInOwl:id>GAZ:00140988</oboInOwl:id>
        <rdfs:label>Avalanche Bay</rdfs:label>
    </owl:NamedIndividual>
    


    <!-- http://purl.obolibrary.org/obo/GAZ_00140991 -->

    <owl:NamedIndividual rdf:about="http://purl.obolibrary.org/obo/GAZ_00140991">
        <obo:RO_0001025 rdf:resource="http://purl.obolibrary.org/obo/GAZ_00051499"/>
        <obo:IAO_0000115>A wide, open bay on the coast between Horn Bluff and Cape Freshfield.</obo:IAO_0000115>
        <oboInOwl:hasOBONamespace>GAZ</oboInOwl:hasOBONamespace>
        <oboInOwl:id>GAZ:00140991</oboInOwl:id>
        <rdfs:label>Deakin Bay</rdfs:label>
    </owl:NamedIndividual>
    


    <!-- http://purl.obolibrary.org/obo/GAZ_00140999 -->

    <owl:NamedIndividual rdf:about="http://purl.obolibrary.org/obo/GAZ_00140999">
        <obo:RO_0001025 rdf:resource="http://purl.obolibrary.org/obo/GAZ_00051499"/>
        <obo:IAO_0000115>An ice-capped island, 10 mi long, lying 4 mi N of Whitmer Peninsula, along the coast of Victoria Land.</obo:IAO_0000115>
        <oboInOwl:hasOBONamespace>GAZ</oboInOwl:hasOBONamespace>
        <oboInOwl:id>GAZ:00140999</oboInOwl:id>
        <rdfs:label>Lamplugh Island</rdfs:label>
    </owl:NamedIndividual>
    


    <!-- http://purl.obolibrary.org/obo/GAZ_00141000 -->

    <owl:NamedIndividual rdf:about="http://purl.obolibrary.org/obo/GAZ_00141000">
        <obo:RO_0001025 rdf:resource="http://purl.obolibrary.org/obo/GAZ_00051499"/>
        <obo:IAO_0000115>A bay indenting the coast of northern Victoria Land between Cape Hooker and Cape Dayman. An inner (western) portion of the bay is circumscribed by Bates Point and Ackroyd Point.</obo:IAO_0000115>
        <oboInOwl:hasOBONamespace>GAZ</oboInOwl:hasOBONamespace>
        <oboInOwl:id>GAZ:00141000</oboInOwl:id>
        <rdfs:label>Yule Bay</rdfs:label>
    </owl:NamedIndividual>
    


    <!-- http://purl.obolibrary.org/obo/GAZ_00141003 -->

    <owl:NamedIndividual rdf:about="http://purl.obolibrary.org/obo/GAZ_00141003">
        <obo:RO_0001025 rdf:resource="http://purl.obolibrary.org/obo/GAZ_00048414"/>
        <obo:IAO_0000115>The northernmost point of Snow Hill Island.</obo:IAO_0000115>
        <oboInOwl:hasOBONamespace>GAZ</oboInOwl:hasOBONamespace>
        <oboInOwl:id>GAZ:00141003</oboInOwl:id>
        <rdfs:label>Cape Lazara</rdfs:label>
    </owl:NamedIndividual>
    


    <!-- http://purl.obolibrary.org/obo/GAZ_00141004 -->

    <owl:NamedIndividual rdf:about="http://purl.obolibrary.org/obo/GAZ_00141004">
        <obo:RO_0001025 rdf:resource="http://purl.obolibrary.org/obo/GAZ_00045042"/>
        <obo:IAO_0000115>An ice-covered peninsula, 30 mi long, which forms the E part of Carney Island, along the coast of Marie Byrd Land.</obo:IAO_0000115>
        <oboInOwl:hasOBONamespace>GAZ</oboInOwl:hasOBONamespace>
        <oboInOwl:id>GAZ:00141004</oboInOwl:id>
        <rdfs:label>Duncan Peninsula</rdfs:label>
    </owl:NamedIndividual>
    


    <!-- http://purl.obolibrary.org/obo/GAZ_00141005 -->

    <owl:NamedIndividual rdf:about="http://purl.obolibrary.org/obo/GAZ_00141005">
        <obo:RO_0001025 rdf:resource="http://purl.obolibrary.org/obo/GAZ_00141004"/>
        <obo:IAO_0000115>An ice-covered cape which marks the north extremity of Duncan Peninsula, Carney Island, along the coast of Marie Byrd Land.</obo:IAO_0000115>
        <oboInOwl:hasOBONamespace>GAZ</oboInOwl:hasOBONamespace>
        <oboInOwl:id>GAZ:00141005</oboInOwl:id>
        <rdfs:label>Cape Leahy</rdfs:label>
    </owl:NamedIndividual>
    


    <!-- http://purl.obolibrary.org/obo/GAZ_00141009 -->

    <owl:NamedIndividual rdf:about="http://purl.obolibrary.org/obo/GAZ_00141009">
        <obo:RO_0001025 rdf:resource="http://purl.obolibrary.org/obo/GAZ_00023304"/>
        <obo:IAO_0000115>A bay about 3 mi wide between Marble Point and Cape Bernacchi, on the coast of Victoria Land.</obo:IAO_0000115>
        <oboInOwl:hasOBONamespace>GAZ</oboInOwl:hasOBONamespace>
        <oboInOwl:id>GAZ:00141009</oboInOwl:id>
        <rdfs:label>Bernacchi Bay</rdfs:label>
    </owl:NamedIndividual>
    


    <!-- http://purl.obolibrary.org/obo/GAZ_00141014 -->

    <owl:NamedIndividual rdf:about="http://purl.obolibrary.org/obo/GAZ_00141014">
        <obo:RO_0001025 rdf:resource="http://purl.obolibrary.org/obo/GAZ_00004045"/>
        <obo:IAO_0000115>An ice-filled inlet 16 mi long, in an E-W direction, and 12 to 15 mi wide, lying between Cape Fanning and Cape Herdman along the E coast of Palmer Land.</obo:IAO_0000115>
        <oboInOwl:hasOBONamespace>GAZ</oboInOwl:hasOBONamespace>
        <oboInOwl:id>GAZ:00141014</oboInOwl:id>
        <rdfs:label>Violante Inlet</rdfs:label>
    </owl:NamedIndividual>
    


    <!-- http://purl.obolibrary.org/obo/GAZ_00141020 -->

    <owl:NamedIndividual rdf:about="http://purl.obolibrary.org/obo/GAZ_00141020">
        <obo:RO_0001025 rdf:resource="http://purl.obolibrary.org/obo/GAZ_00051129"/>
        <obo:IAO_0000115>An open embayment in the vicinity of Gaussberg, just E of the West Ice Shelf.</obo:IAO_0000115>
        <oboInOwl:hasOBONamespace>GAZ</oboInOwl:hasOBONamespace>
        <oboInOwl:id>GAZ:00141020</oboInOwl:id>
        <rdfs:label>Posadowsky Bay</rdfs:label>
    </owl:NamedIndividual>
    


    <!-- http://purl.obolibrary.org/obo/GAZ_00141023 -->

    <owl:NamedIndividual rdf:about="http://purl.obolibrary.org/obo/GAZ_00141023">
        <obo:RO_0001025 rdf:resource="http://purl.obolibrary.org/obo/GAZ_00000373"/>
        <obo:IAO_0000115>A coastal sea between the E end of the Shackleton Ice Shelf, at approximately 105degE and Law Dome, at 113degE. No definitive N boundary. It borders the Knox Coast.</obo:IAO_0000115>
        <oboInOwl:hasOBONamespace>GAZ</oboInOwl:hasOBONamespace>
        <oboInOwl:id>GAZ:00141023</oboInOwl:id>
        <rdfs:label>Mawson Sea</rdfs:label>
    </owl:NamedIndividual>
    


    <!-- http://purl.obolibrary.org/obo/GAZ_00141024 -->

    <owl:NamedIndividual rdf:about="http://purl.obolibrary.org/obo/GAZ_00141024">
        <obo:RO_0001025 rdf:resource="http://purl.obolibrary.org/obo/GAZ_00000373"/>
        <oboInOwl:hasOBONamespace>GAZ</oboInOwl:hasOBONamespace>
        <oboInOwl:id>GAZ:00141024</oboInOwl:id>
        <rdfs:label>Southern Ocean coastal waters of South Orkney Islands</rdfs:label>
    </owl:NamedIndividual>
    


    <!-- http://purl.obolibrary.org/obo/GAZ_00141025 -->

    <owl:NamedIndividual rdf:about="http://purl.obolibrary.org/obo/GAZ_00141025">
        <obo:RO_0001025 rdf:resource="http://purl.obolibrary.org/obo/GAZ_00141023"/>
        <obo:IAO_0000115>A small rocky island lying close to the coast of Antarctica, 13 mi WNW of Cape Nutt.</obo:IAO_0000115>
        <oboInOwl:hasOBONamespace>GAZ</oboInOwl:hasOBONamespace>
        <oboInOwl:id>GAZ:00141025</oboInOwl:id>
        <rdfs:label>Merritt Island</rdfs:label>
    </owl:NamedIndividual>
    


    <!-- http://purl.obolibrary.org/obo/GAZ_00141028 -->

    <owl:NamedIndividual rdf:about="http://purl.obolibrary.org/obo/GAZ_00141028">
        <obo:RO_0001025 rdf:resource="http://purl.obolibrary.org/obo/GAZ_00051499"/>
        <obo:IAO_0000115>An ice-free rock, midway between Cape Bickerton and Rock X, at the E side of the entrance to Victor Bay.</obo:IAO_0000115>
        <oboInOwl:hasOBONamespace>GAZ</oboInOwl:hasOBONamespace>
        <oboInOwl:id>GAZ:00141028</oboInOwl:id>
        <rdfs:label>Mathieu Rock</rdfs:label>
    </owl:NamedIndividual>
    


    <!-- http://purl.obolibrary.org/obo/GAZ_00141029 -->

    <owl:NamedIndividual rdf:about="http://purl.obolibrary.org/obo/GAZ_00141029">
        <obo:RO_0001025 rdf:resource="http://purl.obolibrary.org/obo/GAZ_00051499"/>
        <obo:IAO_0000115>A bay about 16 mi wide and 7 mi long, indenting the coast between Pourquoi Pas Point and Mathieu Rock. The bay is marked by an extensive chain of icebergs breaking away from the high tongue of Commandant Charcot Glacier.</obo:IAO_0000115>
        <oboInOwl:hasOBONamespace>GAZ</oboInOwl:hasOBONamespace>
        <oboInOwl:id>GAZ:00141029</oboInOwl:id>
        <rdfs:label>Victor Bay</rdfs:label>
    </owl:NamedIndividual>
    


    <!-- http://purl.obolibrary.org/obo/GAZ_00141030 -->

    <owl:NamedIndividual rdf:about="http://purl.obolibrary.org/obo/GAZ_00141030">
        <obo:RO_0001025 rdf:resource="http://purl.obolibrary.org/obo/GAZ_00051499"/>
        <obo:IAO_0000115>A prominent offshore rock 0.4 mi long, lying close inside the E side of the entrance to Victor Bay, 1 mi NW of Gravenoire Rock.</obo:IAO_0000115>
        <oboInOwl:hasOBONamespace>GAZ</oboInOwl:hasOBONamespace>
        <oboInOwl:id>GAZ:00141030</oboInOwl:id>
        <rdfs:label>Rock X</rdfs:label>
    </owl:NamedIndividual>
    


    <!-- http://purl.obolibrary.org/obo/GAZ_00141031 -->

    <owl:NamedIndividual rdf:about="http://purl.obolibrary.org/obo/GAZ_00141031">
        <obo:RO_0001025 rdf:resource="http://purl.obolibrary.org/obo/GAZ_00051499"/>
        <obo:IAO_0000115>A small rock outcrop about 1 mi SE of Rock X, protruding above the coastal ice at the E side of Victor Bay.</obo:IAO_0000115>
        <oboInOwl:hasOBONamespace>GAZ</oboInOwl:hasOBONamespace>
        <oboInOwl:id>GAZ:00141031</oboInOwl:id>
        <rdfs:label>Gravenoire Rock</rdfs:label>
    </owl:NamedIndividual>
    


    <!-- http://purl.obolibrary.org/obo/GAZ_00141034 -->

    <owl:NamedIndividual rdf:about="http://purl.obolibrary.org/obo/GAZ_00141034">
        <rdf:type rdf:resource="http://purl.obolibrary.org/obo/ENVO_00000305"/>
        <obo:RO_0001025 rdf:resource="http://purl.obolibrary.org/obo/GAZ_00017734"/>
        <obo:IAO_0000115>A headland forming the east extremity of Snow Island, in the South Shetland Islands.</obo:IAO_0000115>
        <oboInOwl:hasOBONamespace>GAZ</oboInOwl:hasOBONamespace>
        <oboInOwl:id>GAZ:00141034</oboInOwl:id>
        <rdfs:label>President Head</rdfs:label>
    </owl:NamedIndividual>
    


    <!-- http://purl.obolibrary.org/obo/GAZ_00141036 -->

    <owl:NamedIndividual rdf:about="http://purl.obolibrary.org/obo/GAZ_00141036">
        <obo:RO_0001025 rdf:resource="http://purl.obolibrary.org/obo/GAZ_00045055"/>
        <obo:IAO_0000115>A prominent ice-covered headland lying 7 km east of Cape Errera and forming the southeast end of Wiencke Island, in the Palmer Archipelago.</obo:IAO_0000115>
        <oboInOwl:hasOBONamespace>GAZ</oboInOwl:hasOBONamespace>
        <oboInOwl:id>GAZ:00141036</oboInOwl:id>
        <rdfs:label>Principal Point</rdfs:label>
    </owl:NamedIndividual>
    


    <!-- http://purl.obolibrary.org/obo/GAZ_00141037 -->

    <owl:NamedIndividual rdf:about="http://purl.obolibrary.org/obo/GAZ_00141037">
        <rdf:type rdf:resource="http://purl.obolibrary.org/obo/ENVO_00000305"/>
        <obo:RO_0001025 rdf:resource="http://purl.obolibrary.org/obo/GAZ_00045055"/>
        <obo:IAO_0000115>A cape which forms the SW end of Wiencke Island, in the Palmer Archipelago.</obo:IAO_0000115>
        <oboInOwl:hasOBONamespace>GAZ</oboInOwl:hasOBONamespace>
        <oboInOwl:id>GAZ:00141037</oboInOwl:id>
        <rdfs:label>Cape Errera</rdfs:label>
    </owl:NamedIndividual>
    


    <!-- http://purl.obolibrary.org/obo/GAZ_00141038 -->

    <owl:NamedIndividual rdf:about="http://purl.obolibrary.org/obo/GAZ_00141038">
        <obo:RO_0001025 rdf:resource="http://purl.obolibrary.org/obo/GAZ_00023319"/>
        <obo:IAO_0000115>A narrow protruding headland forming the west side of the entrance to Ommanney Bay on the north coast of Coronation Island, in the South Orkney Islands.</obo:IAO_0000115>
        <oboInOwl:hasOBONamespace>GAZ</oboInOwl:hasOBONamespace>
        <oboInOwl:id>GAZ:00141038</oboInOwl:id>
        <rdfs:label>Prong Point</rdfs:label>
    </owl:NamedIndividual>
    


    <!-- http://purl.obolibrary.org/obo/GAZ_00141039 -->

    <owl:NamedIndividual rdf:about="http://purl.obolibrary.org/obo/GAZ_00141039">
        <obo:RO_0001025 rdf:resource="http://purl.obolibrary.org/obo/GAZ_00141024"/>
        <obo:IAO_0000115>A bay 2 mi wide between Prong Point and Foul Point on the N coast of Coronation Island, in the South Orkney Islands.</obo:IAO_0000115>
        <oboInOwl:hasOBONamespace>GAZ</oboInOwl:hasOBONamespace>
        <oboInOwl:id>GAZ:00141039</oboInOwl:id>
        <rdfs:label>Ommanney Bay</rdfs:label>
    </owl:NamedIndividual>
    


    <!-- http://purl.obolibrary.org/obo/GAZ_00141040 -->

    <owl:NamedIndividual rdf:about="http://purl.obolibrary.org/obo/GAZ_00141040">
        <obo:RO_0001025 rdf:resource="http://purl.obolibrary.org/obo/GAZ_00023319"/>
        <obo:IAO_0000115>The N point of the island, with off-lying rocks, lying at the E side of the entrance to Ommanney Bay on the N side of Coronation Island, in the South Orkney Islands.</obo:IAO_0000115>
        <oboInOwl:hasOBONamespace>GAZ</oboInOwl:hasOBONamespace>
        <oboInOwl:id>GAZ:00141040</oboInOwl:id>
        <rdfs:label>Foul Point</rdfs:label>
    </owl:NamedIndividual>
    


    <!-- http://purl.obolibrary.org/obo/GAZ_00141042 -->

    <owl:NamedIndividual rdf:about="http://purl.obolibrary.org/obo/GAZ_00141042">
        <obo:RO_0001025 rdf:resource="http://purl.obolibrary.org/obo/GAZ_00141552"/>
        <obo:IAO_0000115>A bay, 10 mi long in NW-SE direction and averaging 6 mi wide, between Prospect Point and Black Head along the W coast of Graham Land.</obo:IAO_0000115>
        <oboInOwl:hasOBONamespace>GAZ</oboInOwl:hasOBONamespace>
        <oboInOwl:id>GAZ:00141042</oboInOwl:id>
        <rdfs:label>Holtedahl Bay</rdfs:label>
    </owl:NamedIndividual>
    


    <!-- http://purl.obolibrary.org/obo/GAZ_00141043 -->

    <owl:NamedIndividual rdf:about="http://purl.obolibrary.org/obo/GAZ_00141043">
        <obo:RO_0001025 rdf:resource="http://purl.obolibrary.org/obo/GAZ_00141042"/>
        <obo:IAO_0000115>A group of small islands lying in the N part of the entrance to Holtedahl Bay, off the W coast of Graham Land.</obo:IAO_0000115>
        <oboInOwl:hasOBONamespace>GAZ</oboInOwl:hasOBONamespace>
        <oboInOwl:id>GAZ:00141043</oboInOwl:id>
        <rdfs:label>Fish Islands</rdfs:label>
    </owl:NamedIndividual>
    


    <!-- http://purl.obolibrary.org/obo/GAZ_00141051 -->

    <owl:NamedIndividual rdf:about="http://purl.obolibrary.org/obo/GAZ_00141051">
        <rdf:type rdf:resource="http://purl.obolibrary.org/obo/ENVO_00000305"/>
        <obo:RO_0001025 rdf:resource="http://purl.obolibrary.org/obo/GAZ_00004381"/>
        <obo:IAO_0000115>A headland at the north side of the entrance to Perrier Bay, on the northwest coast of Anvers Island in the Palmer Archipelago.</obo:IAO_0000115>
        <oboInOwl:hasOBONamespace>GAZ</oboInOwl:hasOBONamespace>
        <oboInOwl:id>GAZ:00141051</oboInOwl:id>
        <rdfs:label>Quinton Point</rdfs:label>
    </owl:NamedIndividual>
    


    <!-- http://purl.obolibrary.org/obo/GAZ_00141054 -->

    <owl:NamedIndividual rdf:about="http://purl.obolibrary.org/obo/GAZ_00141054">
        <obo:RO_0001025 rdf:resource="http://purl.obolibrary.org/obo/GAZ_00141552"/>
        <obo:IAO_0000115>A bay 6 mi wide indenting the NW coast of Anvers Island between Giard Point and Quinton Point, in the Palmer Archipelago.</obo:IAO_0000115>
        <oboInOwl:hasOBONamespace>GAZ</oboInOwl:hasOBONamespace>
        <oboInOwl:id>GAZ:00141054</oboInOwl:id>
        <rdfs:label>Perrier Bay</rdfs:label>
    </owl:NamedIndividual>
    


    <!-- http://purl.obolibrary.org/obo/GAZ_00141056 -->

    <owl:NamedIndividual rdf:about="http://purl.obolibrary.org/obo/GAZ_00141056">
        <obo:RO_0001025 rdf:resource="http://purl.obolibrary.org/obo/GAZ_00014084"/>
        <obo:IAO_0000115>A bay about 15 mi long and 6 mi wide between Wirth and Rydberg Peninsulas, Ellsworth Land.</obo:IAO_0000115>
        <oboInOwl:hasOBONamespace>GAZ</oboInOwl:hasOBONamespace>
        <oboInOwl:id>GAZ:00141056</oboInOwl:id>
        <rdfs:label>Fladerer Bay</rdfs:label>
    </owl:NamedIndividual>
    


    <!-- http://purl.obolibrary.org/obo/GAZ_00141057 -->

    <owl:NamedIndividual rdf:about="http://purl.obolibrary.org/obo/GAZ_00141057">
        <obo:RO_0001025 rdf:resource="http://purl.obolibrary.org/obo/GAZ_00014084"/>
        <obo:IAO_0000115>An inlet, 40 mi long and 6 mi wide, trending SE along the coast of Ellsworth Land between Rydberg Peninsula and Smyley Island. The head of the inlet is divided into two arms by the presence of Case Island and is bounded to the E by Stange Ice Shelf. Discovered on an airplane flight, 1940-12-22, by members of the USAS (1939-41), and named after Arthur J. Carroll, chief aerial photographer on USAS flights from the East Base.</obo:IAO_0000115>
        <oboInOwl:hasOBONamespace>GAZ</oboInOwl:hasOBONamespace>
        <oboInOwl:id>GAZ:00141057</oboInOwl:id>
        <rdfs:label>Carroll Inlet</rdfs:label>
    </owl:NamedIndividual>
    


    <!-- http://purl.obolibrary.org/obo/GAZ_00141058 -->

    <owl:NamedIndividual rdf:about="http://purl.obolibrary.org/obo/GAZ_00141058">
        <obo:RO_0001025 rdf:resource="http://purl.obolibrary.org/obo/GAZ_00141057"/>
        <obo:IAO_0000115>A roughly circular ice-covered island, 12 mi in diameter, lying off the coast of Ellsworth Land. The island lies in Carroll Inlet between the mainland and Smyley Island.</obo:IAO_0000115>
        <oboInOwl:hasOBONamespace>GAZ</oboInOwl:hasOBONamespace>
        <oboInOwl:id>GAZ:00141058</oboInOwl:id>
        <rdfs:label>Case Island</rdfs:label>
    </owl:NamedIndividual>
    


    <!-- http://purl.obolibrary.org/obo/GAZ_00141060 -->

    <owl:NamedIndividual rdf:about="http://purl.obolibrary.org/obo/GAZ_00141060">
        <obo:RO_0001025 rdf:resource="http://purl.obolibrary.org/obo/GAZ_00014084"/>
        <obo:IAO_0000115>A bay about 35 mi wide in southern Bellingshausen Sea. It indents the coast of Ellsworth Land west of Wirth Peninsula.</obo:IAO_0000115>
        <oboInOwl:hasOBONamespace>GAZ</oboInOwl:hasOBONamespace>
        <oboInOwl:id>GAZ:00141060</oboInOwl:id>
        <rdfs:label>Eltanin Bay</rdfs:label>
    </owl:NamedIndividual>
    


    <!-- http://purl.obolibrary.org/obo/GAZ_00141071 -->

    <owl:NamedIndividual rdf:about="http://purl.obolibrary.org/obo/GAZ_00141071">
        <obo:RO_0001025 rdf:resource="http://purl.obolibrary.org/obo/GAZ_00045019"/>
        <obo:IAO_0000115>Island 2 mi long and 1 mi wide, with three prominent rocky peaks projecting through its icecap, lying 2 mi W of Brooklyn Island in the south-central portion of Wilhelmina Bay, off the W coast of Graham Land.</obo:IAO_0000115>
        <oboInOwl:hasOBONamespace>GAZ</oboInOwl:hasOBONamespace>
        <oboInOwl:id>GAZ:00141071</oboInOwl:id>
        <rdfs:label>Pelseneer Island</rdfs:label>
    </owl:NamedIndividual>
    


    <!-- http://purl.obolibrary.org/obo/GAZ_00141072 -->

    <owl:NamedIndividual rdf:about="http://purl.obolibrary.org/obo/GAZ_00141072">
        <obo:RO_0001025 rdf:resource="http://purl.obolibrary.org/obo/GAZ_00045019"/>
        <obo:IAO_0000115>An island 2.5 mi long, lying 1 mi S of Nansen Island in the E part of Wilhelmina Bay, off the W coast of Graham Land.</obo:IAO_0000115>
        <oboInOwl:hasOBONamespace>GAZ</oboInOwl:hasOBONamespace>
        <oboInOwl:id>GAZ:00141072</oboInOwl:id>
        <rdfs:label>Brooklyn Island</rdfs:label>
    </owl:NamedIndividual>
    


    <!-- http://purl.obolibrary.org/obo/GAZ_00141082 -->

    <owl:NamedIndividual rdf:about="http://purl.obolibrary.org/obo/GAZ_00141082">
        <obo:RO_0001025 rdf:resource="http://purl.obolibrary.org/obo/GAZ_00141552"/>
        <obo:IAO_0000115>A bay 25 mi wide, indenting the W coast of Graham Land between Capes Bellue and Rey.</obo:IAO_0000115>
        <oboInOwl:hasOBONamespace>GAZ</oboInOwl:hasOBONamespace>
        <oboInOwl:id>GAZ:00141082</oboInOwl:id>
        <rdfs:label>Darbel Bay</rdfs:label>
    </owl:NamedIndividual>
    


    <!-- http://purl.obolibrary.org/obo/GAZ_00141083 -->

    <owl:NamedIndividual rdf:about="http://purl.obolibrary.org/obo/GAZ_00141083">
        <obo:RO_0001025 rdf:resource="http://purl.obolibrary.org/obo/GAZ_00141082"/>
        <obo:IAO_0000115>A group of islands and rocks extending SW from Cape Bellue for 5 mi across the entrance to Darbel Bay, off the W coast of Graham Land.</obo:IAO_0000115>
        <oboInOwl:hasOBONamespace>GAZ</oboInOwl:hasOBONamespace>
        <oboInOwl:id>GAZ:00141083</oboInOwl:id>
        <rdfs:label>Darbel Islands</rdfs:label>
    </owl:NamedIndividual>
    


    <!-- http://purl.obolibrary.org/obo/GAZ_00141088 -->

    <owl:NamedIndividual rdf:about="http://purl.obolibrary.org/obo/GAZ_00141088">
        <rdf:type rdf:resource="http://purl.obolibrary.org/obo/ENVO_00000305"/>
        <obo:RO_0001025 rdf:resource="http://purl.obolibrary.org/obo/GAZ_00017732"/>
        <obo:IAO_0000115>A cape forming the northwest extremity of Rugged Island, in the South Shetland Islands.</obo:IAO_0000115>
        <oboInOwl:hasOBONamespace>GAZ</oboInOwl:hasOBONamespace>
        <oboInOwl:id>GAZ:00141088</oboInOwl:id>
        <rdfs:label>Cape Sheffield</rdfs:label>
    </owl:NamedIndividual>
    


    <!-- http://purl.obolibrary.org/obo/GAZ_00141091 -->

    <owl:NamedIndividual rdf:about="http://purl.obolibrary.org/obo/GAZ_00141091">
        <rdf:type rdf:resource="http://purl.obolibrary.org/obo/ENVO_00000305"/>
        <obo:RO_0001025 rdf:resource="http://purl.obolibrary.org/obo/GAZ_00014140"/>
        <obo:IAO_0000115>A headland marked by exposed rock, located 19 km west of Long Glacier on the south coast of Thurston Island.</obo:IAO_0000115>
        <oboInOwl:hasOBONamespace>GAZ</oboInOwl:hasOBONamespace>
        <oboInOwl:id>GAZ:00141091</oboInOwl:id>
        <rdfs:label>Shelton Head</rdfs:label>
    </owl:NamedIndividual>
    


    <!-- http://purl.obolibrary.org/obo/GAZ_00141092 -->

    <owl:NamedIndividual rdf:about="http://purl.obolibrary.org/obo/GAZ_00141092">
        <obo:RO_0001025 rdf:resource="http://purl.obolibrary.org/obo/GAZ_00014140"/>
        <obo:IAO_0000115>A glacier about 8 mi long in the SE part of Thurston Island. It flows S to Abbot Ice Shelf, 14 mi W of Harrison Nunatak.</obo:IAO_0000115>
        <oboInOwl:hasOBONamespace>GAZ</oboInOwl:hasOBONamespace>
        <oboInOwl:id>GAZ:00141092</oboInOwl:id>
        <rdfs:label>Long Glacier</rdfs:label>
    </owl:NamedIndividual>
    


    <!-- http://purl.obolibrary.org/obo/GAZ_00141093 -->

    <owl:NamedIndividual rdf:about="http://purl.obolibrary.org/obo/GAZ_00141093">
        <obo:RO_0001025 rdf:resource="http://purl.obolibrary.org/obo/GAZ_00139150"/>
        <obo:IAO_0000115>A bay 3 mi long and 2 mi wide, indenting the tip of Antarctic Peninsula and opening on Antarctic Sound.</obo:IAO_0000115>
        <oboInOwl:hasOBONamespace>GAZ</oboInOwl:hasOBONamespace>
        <oboInOwl:id>GAZ:00141093</oboInOwl:id>
        <rdfs:label>Hope Bay</rdfs:label>
    </owl:NamedIndividual>
    


    <!-- http://purl.obolibrary.org/obo/GAZ_00141095 -->

    <owl:NamedIndividual rdf:about="http://purl.obolibrary.org/obo/GAZ_00141095">
        <obo:RO_0001025 rdf:resource="http://purl.obolibrary.org/obo/GAZ_00141552"/>
        <obo:IAO_0000115>A high, rugged island 8 km long. It is the largest island of the group which forms the west side of Errera Channel, off the west coast of Graham Land, Antarctica.</obo:IAO_0000115>
        <oboInOwl:hasOBONamespace>GAZ</oboInOwl:hasOBONamespace>
        <oboInOwl:id>GAZ:00141095</oboInOwl:id>
        <rdfs:label>Ronge Island</rdfs:label>
    </owl:NamedIndividual>
    


    <!-- http://purl.obolibrary.org/obo/GAZ_00141096 -->

    <owl:NamedIndividual rdf:about="http://purl.obolibrary.org/obo/GAZ_00141096">
        <obo:RO_0001025 rdf:resource="http://purl.obolibrary.org/obo/GAZ_00141552"/>
        <obo:IAO_0000115>The channel between the W coast of Graham Land and Ronge Island.</obo:IAO_0000115>
        <oboInOwl:hasOBONamespace>GAZ</oboInOwl:hasOBONamespace>
        <oboInOwl:id>GAZ:00141096</oboInOwl:id>
        <rdfs:label>Errera Channel</rdfs:label>
    </owl:NamedIndividual>
    


    <!-- http://purl.obolibrary.org/obo/GAZ_00141097 -->

    <owl:NamedIndividual rdf:about="http://purl.obolibrary.org/obo/GAZ_00141097">
        <rdf:type rdf:resource="http://purl.obolibrary.org/obo/ENVO_00000305"/>
        <obo:RO_0001025 rdf:resource="http://purl.obolibrary.org/obo/GAZ_00141095"/>
        <obo:IAO_0000115>A headland at the southeast end of Ronge Island, off the west coast of Graham Land.</obo:IAO_0000115>
        <oboInOwl:hasOBONamespace>GAZ</oboInOwl:hasOBONamespace>
        <oboInOwl:id>GAZ:00141097</oboInOwl:id>
        <rdfs:label>Sherlac Point</rdfs:label>
    </owl:NamedIndividual>
    


    <!-- http://purl.obolibrary.org/obo/GAZ_00141098 -->

    <owl:NamedIndividual rdf:about="http://purl.obolibrary.org/obo/GAZ_00141098">
        <rdf:type rdf:resource="http://purl.obolibrary.org/obo/ENVO_00000305"/>
        <obo:RO_0001025 rdf:resource="http://purl.obolibrary.org/obo/GAZ_00023349"/>
        <obo:IAO_0000115>A headland at the south end of Astrolabe Island, off Trinity Peninsula.</obo:IAO_0000115>
        <oboInOwl:hasOBONamespace>GAZ</oboInOwl:hasOBONamespace>
        <oboInOwl:id>GAZ:00141098</oboInOwl:id>
        <rdfs:label>Sherrell Point</rdfs:label>
    </owl:NamedIndividual>
    


    <!-- http://purl.obolibrary.org/obo/GAZ_00141116 -->

    <owl:NamedIndividual rdf:about="http://purl.obolibrary.org/obo/GAZ_00141116">
        <obo:RO_0001025 rdf:resource="http://purl.obolibrary.org/obo/GAZ_00139422"/>
        <obo:IAO_0000115>A 3.2 km wide, body of water between Byrd Head and Ufs Island in Antarctica.</obo:IAO_0000115>
        <oboInOwl:hasOBONamespace>GAZ</oboInOwl:hasOBONamespace>
        <oboInOwl:id>GAZ:00141116</oboInOwl:id>
        <rdfs:label>Howard Bay</rdfs:label>
    </owl:NamedIndividual>
    


    <!-- http://purl.obolibrary.org/obo/GAZ_00141117 -->

    <owl:NamedIndividual rdf:about="http://purl.obolibrary.org/obo/GAZ_00141117">
        <obo:RO_0001025 rdf:resource="http://purl.obolibrary.org/obo/GAZ_00141116"/>
        <obo:IAO_0000115>A rocky island 3.2 km wide, lying in the east part of Howard Bay, Antarctica.</obo:IAO_0000115>
        <oboInOwl:hasOBONamespace>GAZ</oboInOwl:hasOBONamespace>
        <oboInOwl:id>GAZ:00141117</oboInOwl:id>
        <rdfs:label>Ufs Island</rdfs:label>
    </owl:NamedIndividual>
    


    <!-- http://purl.obolibrary.org/obo/GAZ_00141118 -->

    <owl:NamedIndividual rdf:about="http://purl.obolibrary.org/obo/GAZ_00141118">
        <obo:RO_0001025 rdf:resource="http://purl.obolibrary.org/obo/GAZ_00141117"/>
        <obo:IAO_0000115>A high rocky bluff at the north end of Ufs Island, forming the east side of the entrance to Howard Bay.</obo:IAO_0000115>
        <oboInOwl:hasOBONamespace>GAZ</oboInOwl:hasOBONamespace>
        <oboInOwl:id>GAZ:00141118</oboInOwl:id>
        <rdfs:label>Cape Simpson</rdfs:label>
    </owl:NamedIndividual>
    


    <!-- http://purl.obolibrary.org/obo/GAZ_00141125 -->

    <owl:NamedIndividual rdf:about="http://purl.obolibrary.org/obo/GAZ_00141125">
        <obo:RO_0001025 rdf:resource="http://purl.obolibrary.org/obo/GAZ_00014085"/>
        <obo:IAO_0000115>An ice-filled inlet about 18 mi long, with two branches, indenting the E end of Thurston Island between Lofgren and Tierney Peninsulas.</obo:IAO_0000115>
        <oboInOwl:hasOBONamespace>GAZ</oboInOwl:hasOBONamespace>
        <oboInOwl:id>GAZ:00141125</oboInOwl:id>
        <rdfs:label>Morgan Inlet</rdfs:label>
    </owl:NamedIndividual>
    


    <!-- http://purl.obolibrary.org/obo/GAZ_00141126 -->

    <owl:NamedIndividual rdf:about="http://purl.obolibrary.org/obo/GAZ_00141126">
        <obo:RO_0001025 rdf:resource="http://purl.obolibrary.org/obo/GAZ_00141125"/>
        <obo:IAO_0000115>An ice-covered island about 2 mi long, lying just within the N part of the mouth of Morgan Inlet, Thurston Island.</obo:IAO_0000115>
        <oboInOwl:hasOBONamespace>GAZ</oboInOwl:hasOBONamespace>
        <oboInOwl:id>GAZ:00141126</oboInOwl:id>
        <rdfs:label>Barrett Island</rdfs:label>
    </owl:NamedIndividual>
    


    <!-- http://purl.obolibrary.org/obo/GAZ_00141127 -->

    <owl:NamedIndividual rdf:about="http://purl.obolibrary.org/obo/GAZ_00141127">
        <obo:RO_0001025 rdf:resource="http://purl.obolibrary.org/obo/GAZ_00014140"/>
        <obo:IAO_0000115>An ice-covered peninsula about 14 mi long, between Savage Glacier and Morgan Inlet in the E end of Thurston Island.</obo:IAO_0000115>
        <oboInOwl:hasOBONamespace>GAZ</oboInOwl:hasOBONamespace>
        <oboInOwl:id>GAZ:00141127</oboInOwl:id>
        <rdfs:label>Tierney Peninsula</rdfs:label>
    </owl:NamedIndividual>
    


    <!-- http://purl.obolibrary.org/obo/GAZ_00141128 -->

    <owl:NamedIndividual rdf:about="http://purl.obolibrary.org/obo/GAZ_00141128">
        <obo:RO_0001025 rdf:resource="http://purl.obolibrary.org/obo/GAZ_00014140"/>
        <obo:IAO_0000115>A glacier at the E end of Thurston Island, lying S of Tierney Peninsula and flowing E to Seraph Bay.</obo:IAO_0000115>
        <oboInOwl:hasOBONamespace>GAZ</oboInOwl:hasOBONamespace>
        <oboInOwl:id>GAZ:00141128</oboInOwl:id>
        <rdfs:label>Savage Glacier</rdfs:label>
    </owl:NamedIndividual>
    


    <!-- http://purl.obolibrary.org/obo/GAZ_00141129 -->

    <owl:NamedIndividual rdf:about="http://purl.obolibrary.org/obo/GAZ_00141129">
        <obo:RO_0001025 rdf:resource="http://purl.obolibrary.org/obo/GAZ_00014140"/>
        <obo:IAO_0000115>An ice-covered peninsula about 22 mi long, projecting between Cadwalader and Morgan Inlets on the NE side of Thurston Island.</obo:IAO_0000115>
        <oboInOwl:hasOBONamespace>GAZ</oboInOwl:hasOBONamespace>
        <oboInOwl:id>GAZ:00141129</oboInOwl:id>
        <rdfs:label>Lofgren Peninsula</rdfs:label>
    </owl:NamedIndividual>
    


    <!-- http://purl.obolibrary.org/obo/GAZ_00141130 -->

    <owl:NamedIndividual rdf:about="http://purl.obolibrary.org/obo/GAZ_00141130">
        <obo:RO_0001025 rdf:resource="http://purl.obolibrary.org/obo/GAZ_00014085"/>
        <obo:IAO_0000115>An ice-filled inlet about 22 mi long, indenting the NE coast of Thurston Island between Evans and Lofgren Peninsulas.</obo:IAO_0000115>
        <oboInOwl:hasOBONamespace>GAZ</oboInOwl:hasOBONamespace>
        <oboInOwl:id>GAZ:00141130</oboInOwl:id>
        <rdfs:label>Cadwalader Inlet</rdfs:label>
    </owl:NamedIndividual>
    


    <!-- http://purl.obolibrary.org/obo/GAZ_00141131 -->

    <owl:NamedIndividual rdf:about="http://purl.obolibrary.org/obo/GAZ_00141131">
        <obo:RO_0001025 rdf:resource="http://purl.obolibrary.org/obo/GAZ_00014140"/>
        <obo:IAO_0000115>An ice-covered peninsula about 30 mi long, between Koether and Cadwalader Inlets in the NE part of Thurston Island.</obo:IAO_0000115>
        <oboInOwl:hasOBONamespace>GAZ</oboInOwl:hasOBONamespace>
        <oboInOwl:id>GAZ:00141131</oboInOwl:id>
        <rdfs:label>Evans Peninsula</rdfs:label>
    </owl:NamedIndividual>
    


    <!-- http://purl.obolibrary.org/obo/GAZ_00141132 -->

    <owl:NamedIndividual rdf:about="http://purl.obolibrary.org/obo/GAZ_00141132">
        <obo:RO_0001025 rdf:resource="http://purl.obolibrary.org/obo/GAZ_00014085"/>
        <obo:IAO_0000115>An ice-filled inlet about 18 mi long, indenting the N coast of Thurston Island between Edwards and Evans Peninsulas.</obo:IAO_0000115>
        <oboInOwl:hasOBONamespace>GAZ</oboInOwl:hasOBONamespace>
        <oboInOwl:id>GAZ:00141132</oboInOwl:id>
        <rdfs:label>Koether Inlet</rdfs:label>
    </owl:NamedIndividual>
    


    <!-- http://purl.obolibrary.org/obo/GAZ_00141133 -->

    <owl:NamedIndividual rdf:about="http://purl.obolibrary.org/obo/GAZ_00141133">
        <obo:RO_0001025 rdf:resource="http://purl.obolibrary.org/obo/GAZ_00014140"/>
        <obo:IAO_0000115>An ice-covered peninsula about 20 mi long, between Murphy and Koether Inlets on the N side of Thurston Island.</obo:IAO_0000115>
        <oboInOwl:hasOBONamespace>GAZ</oboInOwl:hasOBONamespace>
        <oboInOwl:id>GAZ:00141133</oboInOwl:id>
        <rdfs:label>Edwards Peninsula</rdfs:label>
    </owl:NamedIndividual>
    


    <!-- http://purl.obolibrary.org/obo/GAZ_00141134 -->

    <owl:NamedIndividual rdf:about="http://purl.obolibrary.org/obo/GAZ_00141134">
        <obo:RO_0001025 rdf:resource="http://purl.obolibrary.org/obo/GAZ_00014085"/>
        <obo:IAO_0000115>An ice-filled inlet about 18 mi long, with two parallel branches at the head, lying between Noville and Edwards Peninsulas on the N side of Thurston Island.</obo:IAO_0000115>
        <oboInOwl:hasOBONamespace>GAZ</oboInOwl:hasOBONamespace>
        <oboInOwl:id>GAZ:00141134</oboInOwl:id>
        <rdfs:label>Murphy Inlet</rdfs:label>
    </owl:NamedIndividual>
    


    <!-- http://purl.obolibrary.org/obo/GAZ_00141135 -->

    <owl:NamedIndividual rdf:about="http://purl.obolibrary.org/obo/GAZ_00141135">
        <obo:RO_0001025 rdf:resource="http://purl.obolibrary.org/obo/GAZ_00014140"/>
        <obo:IAO_0000115>A high ice-covered peninsula about 30 mi long, between Peale and Murphy Inlets on the N side of Thurston Island.</obo:IAO_0000115>
        <oboInOwl:hasOBONamespace>GAZ</oboInOwl:hasOBONamespace>
        <oboInOwl:id>GAZ:00141135</oboInOwl:id>
        <rdfs:label>Noville Peninsula</rdfs:label>
    </owl:NamedIndividual>
    


    <!-- http://purl.obolibrary.org/obo/GAZ_00141136 -->

    <owl:NamedIndividual rdf:about="http://purl.obolibrary.org/obo/GAZ_00141136">
        <obo:RO_0001025 rdf:resource="http://purl.obolibrary.org/obo/GAZ_00014085"/>
        <obo:IAO_0000115>An ice-filled inlet about 16 mi long, lying immediately W of Noville Peninsula and indenting the N side of Thurston Island.</obo:IAO_0000115>
        <oboInOwl:hasOBONamespace>GAZ</oboInOwl:hasOBONamespace>
        <oboInOwl:id>GAZ:00141136</oboInOwl:id>
        <rdfs:label>Peale Inlet</rdfs:label>
    </owl:NamedIndividual>
    


    <!-- http://purl.obolibrary.org/obo/GAZ_00141137 -->

    <owl:NamedIndividual rdf:about="http://purl.obolibrary.org/obo/GAZ_00141137">
        <obo:RO_0001025 rdf:resource="http://purl.obolibrary.org/obo/GAZ_00014085"/>
        <obo:IAO_0000115>An open bay about 15 mi wide, formed at the SE end of Thurston Island. It is bounded by Cape Annawan on the NW, Abbot Ice Shelf on the SW and Dustin Island on the SE.</obo:IAO_0000115>
        <oboInOwl:hasOBONamespace>GAZ</oboInOwl:hasOBONamespace>
        <oboInOwl:id>GAZ:00141137</oboInOwl:id>
        <rdfs:label>Seraph Bay</rdfs:label>
    </owl:NamedIndividual>
    


    <!-- http://purl.obolibrary.org/obo/GAZ_00141138 -->

    <owl:NamedIndividual rdf:about="http://purl.obolibrary.org/obo/GAZ_00141138">
        <obo:RO_0001025 rdf:resource="http://purl.obolibrary.org/obo/GAZ_00014140"/>
        <obo:IAO_0000115>An ice-covered cape which marks the E extremity of Thurston Island and the NW entrance to Seraph Bay.</obo:IAO_0000115>
        <oboInOwl:hasOBONamespace>GAZ</oboInOwl:hasOBONamespace>
        <oboInOwl:id>GAZ:00141138</oboInOwl:id>
        <rdfs:label>Cape Annawan</rdfs:label>
    </owl:NamedIndividual>
    


    <!-- http://purl.obolibrary.org/obo/GAZ_00141141 -->

    <owl:NamedIndividual rdf:about="http://purl.obolibrary.org/obo/GAZ_00141141">
        <rdf:type rdf:resource="http://purl.obolibrary.org/obo/ENVO_00000305"/>
        <obo:RO_0001025 rdf:resource="http://purl.obolibrary.org/obo/GAZ_00007425"/>
        <obo:IAO_0000115>A headland which forms the W side of the entrance to Admiralty Bay, King George Island, in the South Shetland Islands.</obo:IAO_0000115>
        <oboInOwl:hasOBONamespace>GAZ</oboInOwl:hasOBONamespace>
        <oboInOwl:id>GAZ:00141141</oboInOwl:id>
        <rdfs:label>Demay Point</rdfs:label>
    </owl:NamedIndividual>
    


    <!-- http://purl.obolibrary.org/obo/GAZ_00141142 -->

    <owl:NamedIndividual rdf:about="http://purl.obolibrary.org/obo/GAZ_00141142">
        <obo:RO_0001025 rdf:resource="http://purl.obolibrary.org/obo/GAZ_00007425"/>
        <obo:IAO_0000115>A headland west of the entrance to Admiralty Bay, 3.2 km southwest of Demay Point, King George Island.</obo:IAO_0000115>
        <oboInOwl:hasOBONamespace>GAZ</oboInOwl:hasOBONamespace>
        <oboInOwl:id>GAZ:00141142</oboInOwl:id>
        <rdfs:label>Telefon Point</rdfs:label>
    </owl:NamedIndividual>
    


    <!-- http://purl.obolibrary.org/obo/GAZ_00141143 -->

    <owl:NamedIndividual rdf:about="http://purl.obolibrary.org/obo/GAZ_00141143">
        <obo:RO_0001025 rdf:resource="http://purl.obolibrary.org/obo/GAZ_00007328"/>
        <obo:IAO_0000115>A group of rocks 2.4 km south-southwest of Demay Point, at the west side of the entrance to Admiralty Bay, King George Island, in the South Shetland Islands.</obo:IAO_0000115>
        <oboInOwl:hasOBONamespace>GAZ</oboInOwl:hasOBONamespace>
        <oboInOwl:id>GAZ:00141143</oboInOwl:id>
        <rdfs:label>Telefon Rocks</rdfs:label>
    </owl:NamedIndividual>
    


    <!-- http://purl.obolibrary.org/obo/GAZ_00141144 -->

    <owl:NamedIndividual rdf:about="http://purl.obolibrary.org/obo/GAZ_00141144">
        <obo:RO_0001025 rdf:resource="http://purl.obolibrary.org/obo/GAZ_00045077"/>
        <obo:IAO_0000115>A rocky promontory forming the E extremity of James Ross Island and the W side of the N entrance to Admiralty Sound.</obo:IAO_0000115>
        <oboInOwl:hasOBONamespace>GAZ</oboInOwl:hasOBONamespace>
        <oboInOwl:id>GAZ:00141144</oboInOwl:id>
        <rdfs:label>Cape Gage</rdfs:label>
    </owl:NamedIndividual>
    


    <!-- http://purl.obolibrary.org/obo/GAZ_00141145 -->

    <owl:NamedIndividual rdf:about="http://purl.obolibrary.org/obo/GAZ_00141145">
        <obo:RO_0001025 rdf:resource="http://purl.obolibrary.org/obo/GAZ_00045077"/>
        <obo:IAO_0000115>A low ice-covered point on the northeast coast of James Ross Island, 8 km northwest of Cape Gage.</obo:IAO_0000115>
        <oboInOwl:hasOBONamespace>GAZ</oboInOwl:hasOBONamespace>
        <oboInOwl:id>GAZ:00141145</oboInOwl:id>
        <rdfs:label>Ula Point</rdfs:label>
    </owl:NamedIndividual>
    


    <!-- http://purl.obolibrary.org/obo/GAZ_00141146 -->

    <owl:NamedIndividual rdf:about="http://purl.obolibrary.org/obo/GAZ_00141146">
        <rdf:type rdf:resource="http://purl.obolibrary.org/obo/ENVO_00000305"/>
        <obo:RO_0001025 rdf:resource="http://purl.obolibrary.org/obo/GAZ_00007425"/>
        <obo:IAO_0000115>A headland marking the southwest end of Ullmann Spur in Martel Inlet, Admiralty Bay, on King George Island in the South Shetland Islands.</obo:IAO_0000115>
        <oboInOwl:hasOBONamespace>GAZ</oboInOwl:hasOBONamespace>
        <oboInOwl:id>GAZ:00141146</oboInOwl:id>
        <rdfs:label>Ullmann Point</rdfs:label>
    </owl:NamedIndividual>
    


    <!-- http://purl.obolibrary.org/obo/GAZ_00141147 -->

    <owl:NamedIndividual rdf:about="http://purl.obolibrary.org/obo/GAZ_00141147">
        <obo:RO_0001025 rdf:resource="http://purl.obolibrary.org/obo/GAZ_00140059"/>
        <obo:IAO_0000115>An inlet forming the NE head of Admiralty Bay, King George Island, in the South Shetland Islands.</obo:IAO_0000115>
        <oboInOwl:hasOBONamespace>GAZ</oboInOwl:hasOBONamespace>
        <oboInOwl:id>GAZ:00141147</oboInOwl:id>
        <rdfs:label>Martel Inlet</rdfs:label>
    </owl:NamedIndividual>
    


    <!-- http://purl.obolibrary.org/obo/GAZ_00141149 -->

    <owl:NamedIndividual rdf:about="http://purl.obolibrary.org/obo/GAZ_00141149">
        <obo:RO_0001025 rdf:resource="http://purl.obolibrary.org/obo/GAZ_00045024"/>
        <obo:IAO_0000115>An island 3 mi long, lying W of the S end of Watkins Island, Biscoe Islands.</obo:IAO_0000115>
        <oboInOwl:hasOBONamespace>GAZ</oboInOwl:hasOBONamespace>
        <oboInOwl:id>GAZ:00141149</oboInOwl:id>
        <rdfs:label>Belding Island</rdfs:label>
    </owl:NamedIndividual>
    


    <!-- http://purl.obolibrary.org/obo/GAZ_00141150 -->

    <owl:NamedIndividual rdf:about="http://purl.obolibrary.org/obo/GAZ_00141150">
        <obo:RO_0001025 rdf:resource="http://purl.obolibrary.org/obo/GAZ_00141149"/>
        <obo:IAO_0000115>The northern point of Belding Island, Biscoe Islands.</obo:IAO_0000115>
        <oboInOwl:hasOBONamespace>GAZ</oboInOwl:hasOBONamespace>
        <oboInOwl:id>GAZ:00141150</oboInOwl:id>
        <rdfs:label>Yaglou Point</rdfs:label>
    </owl:NamedIndividual>
    


    <!-- http://purl.obolibrary.org/obo/GAZ_00141153 -->

    <owl:NamedIndividual rdf:about="http://purl.obolibrary.org/obo/GAZ_00141153">
        <obo:RO_0001025 rdf:resource="http://purl.obolibrary.org/obo/GAZ_00051499"/>
        <obo:IAO_0000115>A bay about 12 mi wide, occupied by bay ice and ice shell, indenting the coast between Cape Yevgenov and Coombes Ridge. The Matusevich Glacier Tongue joins Coombes Ridge in forming the W side of the bay.</obo:IAO_0000115>
        <oboInOwl:hasOBONamespace>GAZ</oboInOwl:hasOBONamespace>
        <oboInOwl:id>GAZ:00141153</oboInOwl:id>
        <rdfs:label>Lauritzen Bay</rdfs:label>
    </owl:NamedIndividual>
    


    <!-- http://purl.obolibrary.org/obo/GAZ_00141156 -->

    <owl:NamedIndividual rdf:about="http://purl.obolibrary.org/obo/GAZ_00141156">
        <obo:RO_0001025 rdf:resource="http://purl.obolibrary.org/obo/GAZ_00051499"/>
        <obo:IAO_0000115>A glacier tongue about 18 mi long which is the broad seaward extension of the Matusevich Glacier.</obo:IAO_0000115>
        <oboInOwl:hasOBONamespace>GAZ</oboInOwl:hasOBONamespace>
        <oboInOwl:id>GAZ:00141156</oboInOwl:id>
        <rdfs:label>Matusevich Glacier Tongue</rdfs:label>
    </owl:NamedIndividual>
    


    <!-- http://purl.obolibrary.org/obo/GAZ_00141157 -->

    <owl:NamedIndividual rdf:about="http://purl.obolibrary.org/obo/GAZ_00141157">
        <obo:RO_0001025 rdf:resource="http://purl.obolibrary.org/obo/GAZ_00023304"/>
        <obo:IAO_0000115>An ice-filled reentrant on the W side of the Ross Ice Shelf between Young Head and Harris Point, into which Dickey Glacier flows.</obo:IAO_0000115>
        <oboInOwl:hasOBONamespace>GAZ</oboInOwl:hasOBONamespace>
        <oboInOwl:id>GAZ:00141157</oboInOwl:id>
        <rdfs:label>Beaumont Bay</rdfs:label>
    </owl:NamedIndividual>
    


    <!-- http://purl.obolibrary.org/obo/GAZ_00141199 -->

    <owl:NamedIndividual rdf:about="http://purl.obolibrary.org/obo/GAZ_00141199">
        <obo:RO_0001025 rdf:resource="http://purl.obolibrary.org/obo/GAZ_00014119"/>
        <obo:IAO_0000115>A set of prominent cliffs at about 3,525 m on the north rim of the summit caldera of Mount Erebus, Ross Island.</obo:IAO_0000115>
        <oboInOwl:hasOBONamespace>GAZ</oboInOwl:hasOBONamespace>
        <oboInOwl:id>GAZ:00141199</oboInOwl:id>
        <rdfs:label>Helo Cliffs</rdfs:label>
    </owl:NamedIndividual>
    


    <!-- http://purl.obolibrary.org/obo/GAZ_00141220 -->

    <owl:NamedIndividual rdf:about="http://purl.obolibrary.org/obo/GAZ_00141220">
        <obo:RO_0001025 rdf:resource="http://purl.obolibrary.org/obo/GAZ_00014140"/>
        <obo:IAO_0000115>A broad ice-covered bluff at the east end of Thurston Island. The bluff stands between Levko Glacier and Savage Glacier where they enter Seraph Bay.</obo:IAO_0000115>
        <oboInOwl:hasOBONamespace>GAZ</oboInOwl:hasOBONamespace>
        <oboInOwl:id>GAZ:00141220</oboInOwl:id>
        <rdfs:label>Simpson Bluff</rdfs:label>
    </owl:NamedIndividual>
    


    <!-- http://purl.obolibrary.org/obo/GAZ_00141221 -->

    <owl:NamedIndividual rdf:about="http://purl.obolibrary.org/obo/GAZ_00141221">
        <obo:RO_0001025 rdf:resource="http://purl.obolibrary.org/obo/GAZ_00014140"/>
        <obo:IAO_0000115>A glacier flowing from Pallid Crest to the E end of Thurston Island. It enters Seraph Bay between Tierney Peninsula and Simpson Bluff.</obo:IAO_0000115>
        <oboInOwl:hasOBONamespace>GAZ</oboInOwl:hasOBONamespace>
        <oboInOwl:id>GAZ:00141221</oboInOwl:id>
        <rdfs:label>Levko Glacier</rdfs:label>
    </owl:NamedIndividual>
    


    <!-- http://purl.obolibrary.org/obo/GAZ_00141235 -->

    <owl:NamedIndividual rdf:about="http://purl.obolibrary.org/obo/GAZ_00141235">
        <rdf:type rdf:resource="http://purl.obolibrary.org/obo/ENVO_00000106"/>
        <obo:RO_0001025 rdf:resource="http://purl.obolibrary.org/obo/GAZ_00014140"/>
        <obo:IAO_0000115>A range of peaks and nunataks which are fairly well separated but trend east-west to form the axis, or spine, of Thurston Island.</obo:IAO_0000115>
        <oboInOwl:hasOBONamespace>GAZ</oboInOwl:hasOBONamespace>
        <oboInOwl:id>GAZ:00141235</oboInOwl:id>
        <rdfs:label>Walker Mountains</rdfs:label>
    </owl:NamedIndividual>
    


    <!-- http://purl.obolibrary.org/obo/GAZ_00141236 -->

    <owl:NamedIndividual rdf:about="http://purl.obolibrary.org/obo/GAZ_00141236">
        <obo:RO_0001025 rdf:resource="http://purl.obolibrary.org/obo/GAZ_00141235"/>
        <obo:IAO_0000115>A steep north-facing bluff standing about 8 km east-southeast of Mount Bramhall in the Walker Mountains of Thurston Island.</obo:IAO_0000115>
        <oboInOwl:hasOBONamespace>GAZ</oboInOwl:hasOBONamespace>
        <oboInOwl:id>GAZ:00141236</oboInOwl:id>
        <rdfs:label>Zuhn Bluff</rdfs:label>
    </owl:NamedIndividual>
    


    <!-- http://purl.obolibrary.org/obo/GAZ_00141237 -->

    <owl:NamedIndividual rdf:about="http://purl.obolibrary.org/obo/GAZ_00141237">
        <obo:RO_0001025 rdf:resource="http://purl.obolibrary.org/obo/GAZ_00051499"/>
        <obo:IAO_0000115>An embayment formed between the east side of the Ninnis Glacier Tongue and the mainland of Antarctica.</obo:IAO_0000115>
        <oboInOwl:hasOBONamespace>GAZ</oboInOwl:hasOBONamespace>
        <oboInOwl:id>GAZ:00141237</oboInOwl:id>
        <rdfs:label>Buckley Bay</rdfs:label>
    </owl:NamedIndividual>
    


    <!-- http://purl.obolibrary.org/obo/GAZ_00141238 -->

    <owl:NamedIndividual rdf:about="http://purl.obolibrary.org/obo/GAZ_00141238">
        <obo:RO_0001025 rdf:resource="http://purl.obolibrary.org/obo/GAZ_00141552"/>
        <obo:IAO_0000115>A bay indenting the west coast of Graham Land in a southeast direction for 22 km, between Reclus Peninsula and Cape Murray.</obo:IAO_0000115>
        <oboInOwl:hasOBONamespace>GAZ</oboInOwl:hasOBONamespace>
        <oboInOwl:id>GAZ:00141238</oboInOwl:id>
        <rdfs:label>Charlotte Bay</rdfs:label>
    </owl:NamedIndividual>
    


    <!-- http://purl.obolibrary.org/obo/GAZ_00141240 -->

    <owl:NamedIndividual rdf:about="http://purl.obolibrary.org/obo/GAZ_00141240">
        <obo:RO_0001025 rdf:resource="http://purl.obolibrary.org/obo/GAZ_00014084"/>
        <obo:IAO_0000115>An island 6 mi long lying at the SW side of Hughes Bay, off the W coast of Graham Land.</obo:IAO_0000115>
        <oboInOwl:hasOBONamespace>GAZ</oboInOwl:hasOBONamespace>
        <oboInOwl:id>GAZ:00141240</oboInOwl:id>
        <rdfs:label>Murray Island</rdfs:label>
    </owl:NamedIndividual>
    


    <!-- http://purl.obolibrary.org/obo/GAZ_00141241 -->

    <owl:NamedIndividual rdf:about="http://purl.obolibrary.org/obo/GAZ_00141241">
        <rdf:type rdf:resource="http://purl.obolibrary.org/obo/ENVO_00000305"/>
        <obo:RO_0001025 rdf:resource="http://purl.obolibrary.org/obo/GAZ_00141240"/>
        <obo:IAO_0000115>A cape forming the western end of Murray Island, off the west coast of Graham Land.</obo:IAO_0000115>
        <oboInOwl:hasOBONamespace>GAZ</oboInOwl:hasOBONamespace>
        <oboInOwl:id>GAZ:00141241</oboInOwl:id>
        <rdfs:label>Cape Murray</rdfs:label>
    </owl:NamedIndividual>
    


    <!-- http://purl.obolibrary.org/obo/GAZ_00141242 -->

    <owl:NamedIndividual rdf:about="http://purl.obolibrary.org/obo/GAZ_00141242">
        <obo:RO_0001025 rdf:resource="http://purl.obolibrary.org/obo/GAZ_00014084"/>
        <obo:IAO_0000115>A bay lying between Cape Sterneck and Cape Murray along the W coast of Antarctic Peninsula.</obo:IAO_0000115>
        <oboInOwl:hasOBONamespace>GAZ</oboInOwl:hasOBONamespace>
        <oboInOwl:id>GAZ:00141242</oboInOwl:id>
        <rdfs:label>Hughes Bay</rdfs:label>
    </owl:NamedIndividual>
    


    <!-- http://purl.obolibrary.org/obo/GAZ_00141243 -->

    <owl:NamedIndividual rdf:about="http://purl.obolibrary.org/obo/GAZ_00141243">
        <obo:RO_0001025 rdf:resource="http://purl.obolibrary.org/obo/GAZ_00009523"/>
        <obo:IAO_0000115>A group of small islands 1.2 mi SE of Cape Whitson, off the S coast of Laurie Island in the South Orkney Islands.</obo:IAO_0000115>
        <oboInOwl:hasOBONamespace>GAZ</oboInOwl:hasOBONamespace>
        <oboInOwl:id>GAZ:00141243</oboInOwl:id>
        <rdfs:label>Murray Islands</rdfs:label>
    </owl:NamedIndividual>
    


    <!-- http://purl.obolibrary.org/obo/GAZ_00141245 -->

    <owl:NamedIndividual rdf:about="http://purl.obolibrary.org/obo/GAZ_00141245">
        <obo:RO_0001025 rdf:resource="http://purl.obolibrary.org/obo/GAZ_00141242"/>
        <obo:IAO_0000115>An island lying NW of Charles Point in Hughes Bay, off the W coast of Graham Land.</obo:IAO_0000115>
        <oboInOwl:hasOBONamespace>GAZ</oboInOwl:hasOBONamespace>
        <oboInOwl:id>GAZ:00141245</oboInOwl:id>
        <rdfs:label>Apendice Island</rdfs:label>
    </owl:NamedIndividual>
    


    <!-- http://purl.obolibrary.org/obo/GAZ_00141248 -->

    <owl:NamedIndividual rdf:about="http://purl.obolibrary.org/obo/GAZ_00141248">
        <obo:RO_0001025 rdf:resource="http://purl.obolibrary.org/obo/GAZ_00051133"/>
        <obo:IAO_0000115>A narrow, ice-capped island 3.5 mi long in a N-S direction, marked by ice-free peaks at each end, lying 11 mi SE of Choyce Point, Bowman Coast, in Larsen Ice Shelf.</obo:IAO_0000115>
        <oboInOwl:hasOBONamespace>GAZ</oboInOwl:hasOBONamespace>
        <oboInOwl:id>GAZ:00141248</oboInOwl:id>
        <rdfs:label>Tonkin Island</rdfs:label>
    </owl:NamedIndividual>
    


    <!-- http://purl.obolibrary.org/obo/GAZ_00141250 -->

    <owl:NamedIndividual rdf:about="http://purl.obolibrary.org/obo/GAZ_00141250">
        <obo:RO_0001025 rdf:resource="http://purl.obolibrary.org/obo/GAZ_00139225"/>
        <obo:IAO_0000115>A small bay which indents the Brunt Ice Shelf due west of Halley Station.</obo:IAO_0000115>
        <oboInOwl:hasOBONamespace>GAZ</oboInOwl:hasOBONamespace>
        <oboInOwl:id>GAZ:00141250</oboInOwl:id>
        <rdfs:label>Emperor Bay</rdfs:label>
    </owl:NamedIndividual>
    


    <!-- http://purl.obolibrary.org/obo/GAZ_00141251 -->

    <owl:NamedIndividual rdf:about="http://purl.obolibrary.org/obo/GAZ_00141251">
        <obo:RO_0001025 rdf:resource="http://purl.obolibrary.org/obo/GAZ_00139225"/>
        <obo:IAO_0000115>A British research station located on the Brunt Ice Shelf floating on the Weddell Sea. Established 1956.</obo:IAO_0000115>
        <oboInOwl:hasOBONamespace>GAZ</oboInOwl:hasOBONamespace>
        <oboInOwl:id>GAZ:00141251</oboInOwl:id>
        <rdfs:label>Halley Research Station</rdfs:label>
    </owl:NamedIndividual>
    


    <!-- http://purl.obolibrary.org/obo/GAZ_00141252 -->

    <owl:NamedIndividual rdf:about="http://purl.obolibrary.org/obo/GAZ_00141252">
        <obo:RO_0001025 rdf:resource="http://purl.obolibrary.org/obo/GAZ_00141023"/>
        <obo:IAO_0000115>A bay lying between the west side of Browning Peninsula and the front of Vanderford Glacier at the south end of the Windmill Islands.</obo:IAO_0000115>
        <oboInOwl:hasOBONamespace>GAZ</oboInOwl:hasOBONamespace>
        <oboInOwl:id>GAZ:00141252</oboInOwl:id>
        <rdfs:label>Eyres Bay</rdfs:label>
    </owl:NamedIndividual>
    


    <!-- http://purl.obolibrary.org/obo/GAZ_00141253 -->

    <owl:NamedIndividual rdf:about="http://purl.obolibrary.org/obo/GAZ_00141253">
        <obo:RO_0001025 rdf:resource="http://purl.obolibrary.org/obo/GAZ_00141023"/>
        <obo:IAO_0000115>A large bay extending from Robinson Ridge to Browning Peninsula, at the E side of the Windmill Islands.</obo:IAO_0000115>
        <oboInOwl:hasOBONamespace>GAZ</oboInOwl:hasOBONamespace>
        <oboInOwl:id>GAZ:00141253</oboInOwl:id>
        <rdfs:label>Penney Bay</rdfs:label>
    </owl:NamedIndividual>
    


    <!-- http://purl.obolibrary.org/obo/GAZ_00141254 -->

    <owl:NamedIndividual rdf:about="http://purl.obolibrary.org/obo/GAZ_00141254">
        <obo:RO_0001025 rdf:resource="http://purl.obolibrary.org/obo/GAZ_00141023"/>
        <obo:IAO_0000115>A bay, 1 mi wide and indenting 2.5 mi between Mitchell Peninsula on the N and Robinson Ridge and Odbert Island on the S, in the Windmill Islands.</obo:IAO_0000115>
        <oboInOwl:hasOBONamespace>GAZ</oboInOwl:hasOBONamespace>
        <oboInOwl:id>GAZ:00141254</oboInOwl:id>
        <rdfs:label>Sparkes Bay</rdfs:label>
    </owl:NamedIndividual>
    


    <!-- http://purl.obolibrary.org/obo/GAZ_00141258 -->

    <owl:NamedIndividual rdf:about="http://purl.obolibrary.org/obo/GAZ_00141258">
        <obo:RO_0001025 rdf:resource="http://purl.obolibrary.org/obo/GAZ_00141023"/>
        <obo:IAO_0000115>A bay lying between Bailey and Mitchell Peninsulas on the Budd Coast.</obo:IAO_0000115>
        <oboInOwl:hasOBONamespace>GAZ</oboInOwl:hasOBONamespace>
        <oboInOwl:id>GAZ:00141258</oboInOwl:id>
        <rdfs:label>O&apos;Brien Bay</rdfs:label>
    </owl:NamedIndividual>
    


    <!-- http://purl.obolibrary.org/obo/GAZ_00141260 -->

    <owl:NamedIndividual rdf:about="http://purl.obolibrary.org/obo/GAZ_00141260">
        <obo:RO_0001025 rdf:resource="http://purl.obolibrary.org/obo/GAZ_00045057"/>
        <obo:IAO_0000115>A glacier tongue which extends seaward from Helen Glacier on the coast of Antarctica.</obo:IAO_0000115>
        <oboInOwl:hasOBONamespace>GAZ</oboInOwl:hasOBONamespace>
        <oboInOwl:id>GAZ:00141260</oboInOwl:id>
        <rdfs:label>Helen Glacier Tongue</rdfs:label>
    </owl:NamedIndividual>
    


    <!-- http://purl.obolibrary.org/obo/GAZ_00141261 -->

    <owl:NamedIndividual rdf:about="http://purl.obolibrary.org/obo/GAZ_00141261">
        <obo:RO_0001025 rdf:resource="http://purl.obolibrary.org/obo/GAZ_00045057"/>
        <obo:IAO_0000115>A bay on the coast of Antarctica, 7 miles wide, lying just east of Helen Glacier.</obo:IAO_0000115>
        <oboInOwl:hasOBONamespace>GAZ</oboInOwl:hasOBONamespace>
        <oboInOwl:id>GAZ:00141261</oboInOwl:id>
        <rdfs:label>Farr Bay</rdfs:label>
    </owl:NamedIndividual>
    


    <!-- http://purl.obolibrary.org/obo/GAZ_00141264 -->

    <owl:NamedIndividual rdf:about="http://purl.obolibrary.org/obo/GAZ_00141264">
        <obo:RO_0001025 rdf:resource="http://purl.obolibrary.org/obo/GAZ_00141024"/>
        <obo:IAO_0000115>A cove 1 mi SE of Penguin Point on the N coast of Coronation Island, in the South Orkney Islands.</obo:IAO_0000115>
        <oboInOwl:hasOBONamespace>GAZ</oboInOwl:hasOBONamespace>
        <oboInOwl:id>GAZ:00141264</oboInOwl:id>
        <rdfs:label>Tonsberg Cove</rdfs:label>
    </owl:NamedIndividual>
    


    <!-- http://purl.obolibrary.org/obo/GAZ_00141265 -->

    <owl:NamedIndividual rdf:about="http://purl.obolibrary.org/obo/GAZ_00141265">
        <obo:RO_0001025 rdf:resource="http://purl.obolibrary.org/obo/GAZ_00141024"/>
        <obo:IAO_0000115>A small bay 0.8 km south of Borge Bay along the east side of Signy Island, in the South Orkney Islands.</obo:IAO_0000115>
        <oboInOwl:hasOBONamespace>GAZ</oboInOwl:hasOBONamespace>
        <oboInOwl:id>GAZ:00141265</oboInOwl:id>
        <rdfs:label>Paal Harbor</rdfs:label>
    </owl:NamedIndividual>
    


    <!-- http://purl.obolibrary.org/obo/GAZ_00141266 -->

    <owl:NamedIndividual rdf:about="http://purl.obolibrary.org/obo/GAZ_00141266">
        <obo:RO_0001025 rdf:resource="http://purl.obolibrary.org/obo/GAZ_00141024"/>
        <obo:IAO_0000115>A small bay between Balin and Berntsen Points on the E side of Signy Island, in the South Orkney Islands.</obo:IAO_0000115>
        <oboInOwl:hasOBONamespace>GAZ</oboInOwl:hasOBONamespace>
        <oboInOwl:id>GAZ:00141266</oboInOwl:id>
        <rdfs:label>Borge Bay</rdfs:label>
    </owl:NamedIndividual>
    


    <!-- http://purl.obolibrary.org/obo/GAZ_00141267 -->

    <owl:NamedIndividual rdf:about="http://purl.obolibrary.org/obo/GAZ_00141267">
        <rdf:type rdf:resource="http://purl.obolibrary.org/obo/ENVO_00000305"/>
        <obo:RO_0001025 rdf:resource="http://purl.obolibrary.org/obo/GAZ_00009005"/>
        <obo:IAO_0000115>A headland which marks the N side of the entrance to Borge Bay on the E side of Signy Island, in the South Orkney Islands.</obo:IAO_0000115>
        <oboInOwl:hasOBONamespace>GAZ</oboInOwl:hasOBONamespace>
        <oboInOwl:id>GAZ:00141267</oboInOwl:id>
        <rdfs:label>Balin Point</rdfs:label>
    </owl:NamedIndividual>
    


    <!-- http://purl.obolibrary.org/obo/GAZ_00141268 -->

    <owl:NamedIndividual rdf:about="http://purl.obolibrary.org/obo/GAZ_00141268">
        <rdf:type rdf:resource="http://purl.obolibrary.org/obo/ENVO_00000305"/>
        <obo:RO_0001025 rdf:resource="http://purl.obolibrary.org/obo/GAZ_00009005"/>
        <obo:IAO_0000115>A headland which forms the S side of the entrance to Borge Bay on the E side of Signy Island, in the South Orkney Islands.</obo:IAO_0000115>
        <oboInOwl:hasOBONamespace>GAZ</oboInOwl:hasOBONamespace>
        <oboInOwl:id>GAZ:00141268</oboInOwl:id>
        <rdfs:label>Berntsen Point</rdfs:label>
    </owl:NamedIndividual>
    


    <!-- http://purl.obolibrary.org/obo/GAZ_00141269 -->

    <owl:NamedIndividual rdf:about="http://purl.obolibrary.org/obo/GAZ_00141269">
        <obo:RO_0001025 rdf:resource="http://purl.obolibrary.org/obo/GAZ_00141024"/>
        <obo:IAO_0000115>A small group of rocks close S of Balin Point on the E side of Signy Island, in the South Orkney Islands.</obo:IAO_0000115>
        <oboInOwl:hasOBONamespace>GAZ</oboInOwl:hasOBONamespace>
        <oboInOwl:id>GAZ:00141269</oboInOwl:id>
        <rdfs:label>Balin Rocks</rdfs:label>
    </owl:NamedIndividual>
    


    <!-- http://purl.obolibrary.org/obo/GAZ_00141270 -->

    <owl:NamedIndividual rdf:about="http://purl.obolibrary.org/obo/GAZ_00141270">
        <obo:RO_0001025 rdf:resource="http://purl.obolibrary.org/obo/GAZ_00003703"/>
        <obo:IAO_0000115>A relatively small embayment of the western extremity of the Amery Ice Shelf, about 20 miles northeast of Foley Promontory.</obo:IAO_0000115>
        <oboInOwl:hasOBONamespace>GAZ</oboInOwl:hasOBONamespace>
        <oboInOwl:id>GAZ:00141270</oboInOwl:id>
        <rdfs:label>MacKenzie Bay</rdfs:label>
    </owl:NamedIndividual>
    


    <!-- http://purl.obolibrary.org/obo/GAZ_00141273 -->

    <owl:NamedIndividual rdf:about="http://purl.obolibrary.org/obo/GAZ_00141273">
        <obo:RO_0001025 rdf:resource="http://purl.obolibrary.org/obo/GAZ_00014140"/>
        <obo:IAO_0000115>A glacier about 4 mi long flowing N from the western end of Thurston Island just E of Cape Peterson.</obo:IAO_0000115>
        <oboInOwl:hasOBONamespace>GAZ</oboInOwl:hasOBONamespace>
        <oboInOwl:id>GAZ:00141273</oboInOwl:id>
        <rdfs:label>Foley Glacier</rdfs:label>
    </owl:NamedIndividual>
    


    <!-- http://purl.obolibrary.org/obo/GAZ_00141274 -->

    <owl:NamedIndividual rdf:about="http://purl.obolibrary.org/obo/GAZ_00141274">
        <obo:RO_0001025 rdf:resource="http://purl.obolibrary.org/obo/GAZ_00023294"/>
        <obo:IAO_0000115>A group of small islands, of which Ongul Island is the largest, lying at the E side of the entrance of Lutzow-Holm Bay.</obo:IAO_0000115>
        <oboInOwl:hasOBONamespace>GAZ</oboInOwl:hasOBONamespace>
        <oboInOwl:id>GAZ:00141274</oboInOwl:id>
        <rdfs:label>Flatvaer Islands</rdfs:label>
    </owl:NamedIndividual>
    


    <!-- http://purl.obolibrary.org/obo/GAZ_00141275 -->

    <owl:NamedIndividual rdf:about="http://purl.obolibrary.org/obo/GAZ_00141275">
        <obo:RO_0001025 rdf:resource="http://purl.obolibrary.org/obo/GAZ_00141274"/>
        <obo:IAO_0000115>An island 1.5 mi long, which is the largest feature in the Flatvaer Islands lying just within the E side of the entrance of Lutzow-Holm Bay.</obo:IAO_0000115>
        <oboInOwl:hasOBONamespace>GAZ</oboInOwl:hasOBONamespace>
        <oboInOwl:id>GAZ:00141275</oboInOwl:id>
        <rdfs:label>Ongul Island</rdfs:label>
    </owl:NamedIndividual>
    


    <!-- http://purl.obolibrary.org/obo/GAZ_00141276 -->

    <owl:NamedIndividual rdf:about="http://purl.obolibrary.org/obo/GAZ_00141276">
        <obo:RO_0001025 rdf:resource="http://purl.obolibrary.org/obo/GAZ_00141274"/>
        <obo:IAO_0000115>An island, 1 mi long, lying immediately E of the N part of Ongul Island at the E side of the entrance of Lutzow-Holm Bay.</obo:IAO_0000115>
        <oboInOwl:hasOBONamespace>GAZ</oboInOwl:hasOBONamespace>
        <oboInOwl:id>GAZ:00141276</oboInOwl:id>
        <rdfs:label>East Ongul Island</rdfs:label>
    </owl:NamedIndividual>
    


    <!-- http://purl.obolibrary.org/obo/GAZ_00141277 -->

    <owl:NamedIndividual rdf:about="http://purl.obolibrary.org/obo/GAZ_00141277">
        <obo:RO_0001025 rdf:resource="http://purl.obolibrary.org/obo/GAZ_00141274"/>
        <obo:IAO_0000115>An island lying 1 mi W of Ongul Island in Lutzow-Holm Bay.</obo:IAO_0000115>
        <oboInOwl:hasOBONamespace>GAZ</oboInOwl:hasOBONamespace>
        <oboInOwl:id>GAZ:00141277</oboInOwl:id>
        <rdfs:label>Ongulkalven Island</rdfs:label>
    </owl:NamedIndividual>
    


    <!-- http://purl.obolibrary.org/obo/GAZ_00141278 -->

    <owl:NamedIndividual rdf:about="http://purl.obolibrary.org/obo/GAZ_00141278">
        <obo:RO_0001025 rdf:resource="http://purl.obolibrary.org/obo/GAZ_00023294"/>
        <obo:IAO_0000115>A sound, 2 mi wide, between the E shore of Lutzow-Holm Bay and the Flatvaer Islands in which Ongul Island is the principal feature.</obo:IAO_0000115>
        <oboInOwl:hasOBONamespace>GAZ</oboInOwl:hasOBONamespace>
        <oboInOwl:id>GAZ:00141278</oboInOwl:id>
        <rdfs:label>Ongul Sound</rdfs:label>
    </owl:NamedIndividual>
    


    <!-- http://purl.obolibrary.org/obo/GAZ_00141279 -->

    <owl:NamedIndividual rdf:about="http://purl.obolibrary.org/obo/GAZ_00141279">
        <obo:RO_0001025 rdf:resource="http://purl.obolibrary.org/obo/GAZ_00141274"/>
        <obo:IAO_0000115>The northernmost of three aligned islands lying 1 mi SE of the Te Islands, at the S end of the Flatvaer Islands.</obo:IAO_0000115>
        <oboInOwl:hasOBONamespace>GAZ</oboInOwl:hasOBONamespace>
        <oboInOwl:id>GAZ:00141279</oboInOwl:id>
        <rdfs:label>Ongulgalten Island</rdfs:label>
    </owl:NamedIndividual>
    


    <!-- http://purl.obolibrary.org/obo/GAZ_00141280 -->

    <owl:NamedIndividual rdf:about="http://purl.obolibrary.org/obo/GAZ_00141280">
        <obo:RO_0001025 rdf:resource="http://purl.obolibrary.org/obo/GAZ_00141274"/>
        <obo:IAO_0000115>Three small islands and several rocks lying close together just S of Ongul Island in the Flatvaer Islands.</obo:IAO_0000115>
        <oboInOwl:hasOBONamespace>GAZ</oboInOwl:hasOBONamespace>
        <oboInOwl:id>GAZ:00141280</oboInOwl:id>
        <rdfs:label>Te Islands</rdfs:label>
    </owl:NamedIndividual>
    


    <!-- http://purl.obolibrary.org/obo/GAZ_00141282 -->

    <owl:NamedIndividual rdf:about="http://purl.obolibrary.org/obo/GAZ_00141282">
        <obo:RO_0001025 rdf:resource="http://purl.obolibrary.org/obo/GAZ_00051499"/>
        <obo:IAO_0000115>A small bay bordering the east side of Cape Decouverte.</obo:IAO_0000115>
        <oboInOwl:hasOBONamespace>GAZ</oboInOwl:hasOBONamespace>
        <oboInOwl:id>GAZ:00141282</oboInOwl:id>
        <rdfs:label>Ionosphere Bay</rdfs:label>
    </owl:NamedIndividual>
    


    <!-- http://purl.obolibrary.org/obo/GAZ_00141284 -->

    <owl:NamedIndividual rdf:about="http://purl.obolibrary.org/obo/GAZ_00141284">
        <obo:RO_0001025 rdf:resource="http://purl.obolibrary.org/obo/GAZ_00141552"/>
        <obo:IAO_0000115>A small bay between Andrews Point and Briggs Peninsula along the northeast coast of Anvers Island, in the Palmer Archipelago.</obo:IAO_0000115>
        <oboInOwl:hasOBONamespace>GAZ</oboInOwl:hasOBONamespace>
        <oboInOwl:id>GAZ:00141284</oboInOwl:id>
        <rdfs:label>Inverleith Harbor</rdfs:label>
    </owl:NamedIndividual>
    


    <!-- http://purl.obolibrary.org/obo/GAZ_00141285 -->

    <owl:NamedIndividual rdf:about="http://purl.obolibrary.org/obo/GAZ_00141285">
        <obo:RO_0001025 rdf:resource="http://purl.obolibrary.org/obo/GAZ_00004381"/>
        <obo:IAO_0000115>A small peninsula forming the W side of Inverleith Harbor on the NE coast of Anvers Island, in the Palmer Archipelago.</obo:IAO_0000115>
        <oboInOwl:hasOBONamespace>GAZ</oboInOwl:hasOBONamespace>
        <oboInOwl:id>GAZ:00141285</oboInOwl:id>
        <rdfs:label>Briggs Peninsula</rdfs:label>
    </owl:NamedIndividual>
    


    <!-- http://purl.obolibrary.org/obo/GAZ_00141286 -->

    <owl:NamedIndividual rdf:about="http://purl.obolibrary.org/obo/GAZ_00141286">
        <rdf:type rdf:resource="http://purl.obolibrary.org/obo/ENVO_00000305"/>
        <obo:RO_0001025 rdf:resource="http://purl.obolibrary.org/obo/GAZ_00004381"/>
        <obo:IAO_0000115>A headland between Hackapike Bay and Inverleith Harbor on the NE coast of Anvers Island, in the Palmer Archipelago.</obo:IAO_0000115>
        <oboInOwl:hasOBONamespace>GAZ</oboInOwl:hasOBONamespace>
        <oboInOwl:id>GAZ:00141286</oboInOwl:id>
        <rdfs:label>Andrews Point</rdfs:label>
    </owl:NamedIndividual>
    


    <!-- http://purl.obolibrary.org/obo/GAZ_00141287 -->

    <owl:NamedIndividual rdf:about="http://purl.obolibrary.org/obo/GAZ_00141287">
        <obo:RO_0001025 rdf:resource="http://purl.obolibrary.org/obo/GAZ_00141552"/>
        <obo:IAO_0000115>An anchorage 6 km northwest of Ryswyck Point, entered west of False Island along the northeast coast of Anvers Island, in the Palmer Archipelago.</obo:IAO_0000115>
        <oboInOwl:hasOBONamespace>GAZ</oboInOwl:hasOBONamespace>
        <oboInOwl:id>GAZ:00141287</oboInOwl:id>
        <rdfs:label>Hackapike Bay</rdfs:label>
    </owl:NamedIndividual>
    


    <!-- http://purl.obolibrary.org/obo/GAZ_00141288 -->

    <owl:NamedIndividual rdf:about="http://purl.obolibrary.org/obo/GAZ_00141288">
        <obo:RO_0001025 rdf:resource="http://purl.obolibrary.org/obo/GAZ_00141287"/>
        <obo:IAO_0000115>The largest of three islands lying at the E side of Hackapike Bay, off the NE coast of Anvers Island, in the Palmer Archipelago.</obo:IAO_0000115>
        <oboInOwl:hasOBONamespace>GAZ</oboInOwl:hasOBONamespace>
        <oboInOwl:id>GAZ:00141288</oboInOwl:id>
        <rdfs:label>False Island</rdfs:label>
    </owl:NamedIndividual>
    


    <!-- http://purl.obolibrary.org/obo/GAZ_00141289 -->

    <owl:NamedIndividual rdf:about="http://purl.obolibrary.org/obo/GAZ_00141289">
        <rdf:type rdf:resource="http://purl.obolibrary.org/obo/ENVO_00000305"/>
        <obo:RO_0001025 rdf:resource="http://purl.obolibrary.org/obo/GAZ_00045106"/>
        <obo:IAO_0000115>A headland 1 mi long and 0.5 mi wide, which is connected by a low, narrow, almost invisible isthmus to the S side of Vega Island, lying S of the NE end of Antarctic Peninsula.</obo:IAO_0000115>
        <oboInOwl:hasOBONamespace>GAZ</oboInOwl:hasOBONamespace>
        <oboInOwl:id>GAZ:00141289</oboInOwl:id>
        <rdfs:label>False Island Point</rdfs:label>
    </owl:NamedIndividual>
    


    <!-- http://purl.obolibrary.org/obo/GAZ_00141290 -->

    <owl:NamedIndividual rdf:about="http://purl.obolibrary.org/obo/GAZ_00141290">
        <obo:RO_0001025 rdf:resource="http://purl.obolibrary.org/obo/GAZ_00004045"/>
        <obo:IAO_0000115>A bay lying immediately east of Mount Alexander along the south coast of Joinville Island, Antarctica.</obo:IAO_0000115>
        <oboInOwl:hasOBONamespace>GAZ</oboInOwl:hasOBONamespace>
        <oboInOwl:id>GAZ:00141290</oboInOwl:id>
        <rdfs:label>Haddon Bay</rdfs:label>
    </owl:NamedIndividual>
    


    <!-- http://purl.obolibrary.org/obo/GAZ_00141292 -->

    <owl:NamedIndividual rdf:about="http://purl.obolibrary.org/obo/GAZ_00141292">
        <obo:RO_0001025 rdf:resource="http://purl.obolibrary.org/obo/GAZ_00139496"/>
        <obo:IAO_0000115>A bay on the southwest side of Port Foster, Deception Island, in the South Shetland Islands.</obo:IAO_0000115>
        <oboInOwl:hasOBONamespace>GAZ</oboInOwl:hasOBONamespace>
        <oboInOwl:id>GAZ:00141292</oboInOwl:id>
        <rdfs:label>Primero de Mayo Bay</rdfs:label>
    </owl:NamedIndividual>
    


    <!-- http://purl.obolibrary.org/obo/GAZ_00141293 -->

    <owl:NamedIndividual rdf:about="http://purl.obolibrary.org/obo/GAZ_00141293">
        <rdf:type rdf:resource="http://purl.obolibrary.org/obo/ENVO_00000032"/>
        <obo:RO_0001025 rdf:resource="http://purl.obolibrary.org/obo/GAZ_00141554"/>
        <obo:IAO_0000115>A bight 30 mi wide, indenting the ice shelf that fringes the coast of Queen Maud Land about 20 mi NE of Tsiolkovskiy Island.</obo:IAO_0000115>
        <oboInOwl:hasOBONamespace>GAZ</oboInOwl:hasOBONamespace>
        <oboInOwl:id>GAZ:00141293</oboInOwl:id>
        <rdfs:label>Neupokoyev Bight</rdfs:label>
    </owl:NamedIndividual>
    


    <!-- http://purl.obolibrary.org/obo/GAZ_00141294 -->

    <owl:NamedIndividual rdf:about="http://purl.obolibrary.org/obo/GAZ_00141294">
        <obo:RO_0001025 rdf:resource="http://purl.obolibrary.org/obo/GAZ_00141293"/>
        <obo:IAO_0000115>A bay that indents the southwest side of Neupokoyev Bight, along the ice shelf that fringes the coast of Queen Maud Land.</obo:IAO_0000115>
        <oboInOwl:hasOBONamespace>GAZ</oboInOwl:hasOBONamespace>
        <oboInOwl:id>GAZ:00141294</oboInOwl:id>
        <rdfs:label>Proshchaniya Bay</rdfs:label>
    </owl:NamedIndividual>
    


    <!-- http://purl.obolibrary.org/obo/GAZ_00141295 -->

    <owl:NamedIndividual rdf:about="http://purl.obolibrary.org/obo/GAZ_00141295">
        <obo:RO_0001025 rdf:resource="http://purl.obolibrary.org/obo/GAZ_00139488"/>
        <obo:IAO_0000115>An ice-covered island in the Fimbul Ice Shelf, Queen Maud Land.</obo:IAO_0000115>
        <oboInOwl:hasOBONamespace>GAZ</oboInOwl:hasOBONamespace>
        <oboInOwl:id>GAZ:00141295</oboInOwl:id>
        <rdfs:label>Tsiolkovskiy Island</rdfs:label>
    </owl:NamedIndividual>
    


    <!-- http://purl.obolibrary.org/obo/GAZ_00141296 -->

    <owl:NamedIndividual rdf:about="http://purl.obolibrary.org/obo/GAZ_00141296">
        <obo:RO_0001025 rdf:resource="http://purl.obolibrary.org/obo/GAZ_00141293"/>
        <obo:IAO_0000115>A small bay that indents the southeast side of Neupokoyev Bight, along the ice shelf that fringes the coast of Queen Maud Land.</obo:IAO_0000115>
        <oboInOwl:hasOBONamespace>GAZ</oboInOwl:hasOBONamespace>
        <oboInOwl:id>GAZ:00141296</oboInOwl:id>
        <rdfs:label>Pryamougol&apos;naya Bay</rdfs:label>
    </owl:NamedIndividual>
    


    <!-- http://purl.obolibrary.org/obo/GAZ_00141297 -->

    <owl:NamedIndividual rdf:about="http://purl.obolibrary.org/obo/GAZ_00141297">
        <obo:RO_0001025 rdf:resource="http://purl.obolibrary.org/obo/GAZ_00014085"/>
        <obo:IAO_0000115>A rather open bay in southwestern Amundsen Sea, extending along the north sides of Siple Island, Getz Ice Shelf and Carney Island, from Pranke Island to Cape Gates.</obo:IAO_0000115>
        <oboInOwl:hasOBONamespace>GAZ</oboInOwl:hasOBONamespace>
        <oboInOwl:id>GAZ:00141297</oboInOwl:id>
        <rdfs:label>Russell Bay</rdfs:label>
    </owl:NamedIndividual>
    


    <!-- http://purl.obolibrary.org/obo/GAZ_00141301 -->

    <owl:NamedIndividual rdf:about="http://purl.obolibrary.org/obo/GAZ_00141301">
        <obo:RO_0001025 rdf:resource="http://purl.obolibrary.org/obo/GAZ_00140467"/>
        <obo:IAO_0000115>A bay which indents the northeastern end of Riiser-Larsen Ice Shelf just southward of Cape Norvegia, on the coast of Queen Maud Land.</obo:IAO_0000115>
        <oboInOwl:hasOBONamespace>GAZ</oboInOwl:hasOBONamespace>
        <oboInOwl:id>GAZ:00141301</oboInOwl:id>
        <rdfs:label>Seal Bay</rdfs:label>
    </owl:NamedIndividual>
    


    <!-- http://purl.obolibrary.org/obo/GAZ_00141302 -->

    <owl:NamedIndividual rdf:about="http://purl.obolibrary.org/obo/GAZ_00141302">
        <obo:RO_0001025 rdf:resource="http://purl.obolibrary.org/obo/GAZ_00140059"/>
        <obo:IAO_0000115>A bay between Cape Melville and Penguin Island on the south side of King George Island, in the South Shetland Islands.</obo:IAO_0000115>
        <oboInOwl:hasOBONamespace>GAZ</oboInOwl:hasOBONamespace>
        <oboInOwl:id>GAZ:00141302</oboInOwl:id>
        <rdfs:label>Sherratt Bay</rdfs:label>
    </owl:NamedIndividual>
    


    <!-- http://purl.obolibrary.org/obo/GAZ_00141303 -->

    <owl:NamedIndividual rdf:about="http://purl.obolibrary.org/obo/GAZ_00141303">
        <obo:RO_0001025 rdf:resource="http://purl.obolibrary.org/obo/GAZ_00007425"/>
        <obo:IAO_0000115>The cape forming the E extremity of King George Island, in the South Shetland Islands.</obo:IAO_0000115>
        <oboInOwl:hasOBONamespace>GAZ</oboInOwl:hasOBONamespace>
        <oboInOwl:id>GAZ:00141303</oboInOwl:id>
        <rdfs:label>Cape Melville</rdfs:label>
    </owl:NamedIndividual>
    


    <!-- http://purl.obolibrary.org/obo/GAZ_00141304 -->

    <owl:NamedIndividual rdf:about="http://purl.obolibrary.org/obo/GAZ_00141304">
        <obo:RO_0001025 rdf:resource="http://purl.obolibrary.org/obo/GAZ_00004045"/>
        <obo:IAO_0000115>A small bay indenting the west end of Joinville Island just south of Madder Cliffs.</obo:IAO_0000115>
        <oboInOwl:hasOBONamespace>GAZ</oboInOwl:hasOBONamespace>
        <oboInOwl:id>GAZ:00141304</oboInOwl:id>
        <rdfs:label>Suspiros Bay</rdfs:label>
    </owl:NamedIndividual>
    


    <!-- http://purl.obolibrary.org/obo/GAZ_00141305 -->

    <owl:NamedIndividual rdf:about="http://purl.obolibrary.org/obo/GAZ_00141305">
        <obo:RO_0001025 rdf:resource="http://purl.obolibrary.org/obo/GAZ_00004044"/>
        <obo:IAO_0000115>Reddish rock cliffs rising steeply from the sea to about 305 m and forming the N side of the entrance to Suspiros Bay, at the W end of Joinville Island.</obo:IAO_0000115>
        <oboInOwl:hasOBONamespace>GAZ</oboInOwl:hasOBONamespace>
        <oboInOwl:id>GAZ:00141305</oboInOwl:id>
        <rdfs:label>Madder Cliffs</rdfs:label>
    </owl:NamedIndividual>
    


    <!-- http://purl.obolibrary.org/obo/GAZ_00141306 -->

    <owl:NamedIndividual rdf:about="http://purl.obolibrary.org/obo/GAZ_00141306">
        <rdf:type rdf:resource="http://purl.obolibrary.org/obo/ENVO_00000305"/>
        <obo:RO_0001025 rdf:resource="http://purl.obolibrary.org/obo/GAZ_00014121"/>
        <obo:IAO_0000115>A headland which forms the N side of Neptunes Bellows, the entrance to Port Foster, Deception Island, in the South Shetland Islands.</obo:IAO_0000115>
        <oboInOwl:hasOBONamespace>GAZ</oboInOwl:hasOBONamespace>
        <oboInOwl:id>GAZ:00141306</oboInOwl:id>
        <rdfs:label>Fildes Point</rdfs:label>
    </owl:NamedIndividual>
    


    <!-- http://purl.obolibrary.org/obo/GAZ_00141307 -->

    <owl:NamedIndividual rdf:about="http://purl.obolibrary.org/obo/GAZ_00141307">
        <rdf:type rdf:resource="http://purl.obolibrary.org/obo/ENVO_00000305"/>
        <obo:RO_0001025 rdf:resource="http://purl.obolibrary.org/obo/GAZ_00014121"/>
        <obo:IAO_0000115>A headland which forms the NW side of the entrance to Whalers Bay, Deception Island, in the South Shetland Islands.</obo:IAO_0000115>
        <oboInOwl:hasOBONamespace>GAZ</oboInOwl:hasOBONamespace>
        <oboInOwl:id>GAZ:00141307</oboInOwl:id>
        <rdfs:label>Penfold Point</rdfs:label>
    </owl:NamedIndividual>
    


    <!-- http://purl.obolibrary.org/obo/GAZ_00141308 -->

    <owl:NamedIndividual rdf:about="http://purl.obolibrary.org/obo/GAZ_00141308">
        <obo:RO_0001025 rdf:resource="http://purl.obolibrary.org/obo/GAZ_00007328"/>
        <obo:IAO_0000115>A rock, 105 m high, lying 0.75 mi off the SW coast of Deception Island, in the South Shetland Islands.</obo:IAO_0000115>
        <oboInOwl:hasOBONamespace>GAZ</oboInOwl:hasOBONamespace>
        <oboInOwl:id>GAZ:00141308</oboInOwl:id>
        <rdfs:label>New Rock</rdfs:label>
    </owl:NamedIndividual>
    


    <!-- http://purl.obolibrary.org/obo/GAZ_00141309 -->

    <owl:NamedIndividual rdf:about="http://purl.obolibrary.org/obo/GAZ_00141309">
        <obo:RO_0001025 rdf:resource="http://purl.obolibrary.org/obo/GAZ_00139496"/>
        <obo:IAO_0000115>A cove NE of Laguna Hill in the NW part of Port Foster, Deception Island, in the South Shetland Islands. The feature was formed as the result of volcanic eruptions on the island between 1967-12 and 1970-08.</obo:IAO_0000115>
        <oboInOwl:hasOBONamespace>GAZ</oboInOwl:hasOBONamespace>
        <oboInOwl:id>GAZ:00141309</oboInOwl:id>
        <rdfs:label>Stancomb Cove</rdfs:label>
    </owl:NamedIndividual>
    


    <!-- http://purl.obolibrary.org/obo/GAZ_00141310 -->

    <owl:NamedIndividual rdf:about="http://purl.obolibrary.org/obo/GAZ_00141310">
        <obo:RO_0001025 rdf:resource="http://purl.obolibrary.org/obo/GAZ_00141311"/>
        <obo:IAO_0000115>A volcanic crater, now filled with water, lying NW of Mount Kirkwood on the S side of Deception Island, in the South Shetland Islands.</obo:IAO_0000115>
        <oboInOwl:hasOBONamespace>GAZ</oboInOwl:hasOBONamespace>
        <oboInOwl:id>GAZ:00141310</oboInOwl:id>
        <rdfs:label>Crater Lake</rdfs:label>
    </owl:NamedIndividual>
    


    <!-- http://purl.obolibrary.org/obo/GAZ_00141311 -->

    <owl:NamedIndividual rdf:about="http://purl.obolibrary.org/obo/GAZ_00141311">
        <obo:RO_0001025 rdf:resource="http://purl.obolibrary.org/obo/GAZ_00014121"/>
        <obo:IAO_0000115>A mountain, 460 m, standing 3 mi W of Entrance Point in the S part of Deception Island, in the South Shetland Islands.</obo:IAO_0000115>
        <oboInOwl:hasOBONamespace>GAZ</oboInOwl:hasOBONamespace>
        <oboInOwl:id>GAZ:00141311</oboInOwl:id>
        <rdfs:label>Mount Kirkwood</rdfs:label>
    </owl:NamedIndividual>
    


    <!-- http://purl.obolibrary.org/obo/GAZ_00141312 -->

    <owl:NamedIndividual rdf:about="http://purl.obolibrary.org/obo/GAZ_00141312">
        <obo:RO_0001025 rdf:resource="http://purl.obolibrary.org/obo/GAZ_00014089"/>
        <obo:IAO_0000115>A scattered group of reefs and rocks, with one larger island, lying in the central part of Marguerite Bay, 15 mi SSW of the Faure Islands.</obo:IAO_0000115>
        <oboInOwl:hasOBONamespace>GAZ</oboInOwl:hasOBONamespace>
        <oboInOwl:id>GAZ:00141312</oboInOwl:id>
        <rdfs:label>Kirkwood Islands</rdfs:label>
    </owl:NamedIndividual>
    


    <!-- http://purl.obolibrary.org/obo/GAZ_00141313 -->

    <owl:NamedIndividual rdf:about="http://purl.obolibrary.org/obo/GAZ_00141313">
        <obo:RO_0001025 rdf:resource="http://purl.obolibrary.org/obo/GAZ_00014121"/>
        <obo:IAO_0000115>A circular lake 0.2 mi in diameter lying immediately W of Whalers Bay, on Deception Island in the South Shetland Islands.</obo:IAO_0000115>
        <oboInOwl:hasOBONamespace>GAZ</oboInOwl:hasOBONamespace>
        <oboInOwl:id>GAZ:00141313</oboInOwl:id>
        <rdfs:label>Kroner Lake</rdfs:label>
    </owl:NamedIndividual>
    


    <!-- http://purl.obolibrary.org/obo/GAZ_00141314 -->

    <owl:NamedIndividual rdf:about="http://purl.obolibrary.org/obo/GAZ_00141314">
        <obo:RO_0001025 rdf:resource="http://purl.obolibrary.org/obo/GAZ_00007328"/>
        <obo:IAO_0000115>A small island S of Deception Island.</obo:IAO_0000115>
        <oboInOwl:hasOBONamespace>GAZ</oboInOwl:hasOBONamespace>
        <oboInOwl:id>GAZ:00141314</oboInOwl:id>
        <rdfs:label>Lavebrua Island</rdfs:label>
    </owl:NamedIndividual>
    


    <!-- http://purl.obolibrary.org/obo/GAZ_00141315 -->

    <owl:NamedIndividual rdf:about="http://purl.obolibrary.org/obo/GAZ_00141315">
        <obo:RO_0001025 rdf:resource="http://purl.obolibrary.org/obo/GAZ_00011769"/>
        <obo:IAO_0000115>An iceport indenting the front of Ross Ice Shelf just northward of Roosevelt Island.</obo:IAO_0000115>
        <oboInOwl:hasOBONamespace>GAZ</oboInOwl:hasOBONamespace>
        <oboInOwl:id>GAZ:00141315</oboInOwl:id>
        <rdfs:label>Bay of Whales</rdfs:label>
    </owl:NamedIndividual>
    


    <!-- http://purl.obolibrary.org/obo/GAZ_00141318 -->

    <owl:NamedIndividual rdf:about="http://purl.obolibrary.org/obo/GAZ_00141318">
        <obo:RO_0001025 rdf:resource="http://purl.obolibrary.org/obo/GAZ_00002625"/>
        <obo:IAO_0000115>A small cove of McMurdo Sound, Antarctica.</obo:IAO_0000115>
        <oboInOwl:hasOBONamespace>GAZ</oboInOwl:hasOBONamespace>
        <oboInOwl:id>GAZ:00141318</oboInOwl:id>
        <rdfs:label>Winter Quarters Bay</rdfs:label>
    </owl:NamedIndividual>
    


    <!-- http://purl.obolibrary.org/obo/GAZ_00141319 -->

    <owl:NamedIndividual rdf:about="http://purl.obolibrary.org/obo/GAZ_00141319">
        <obo:RO_0001025 rdf:resource="http://purl.obolibrary.org/obo/GAZ_00141552"/>
        <obo:IAO_0000115>A bay 4.0 km wide, indenting the east side of Renaud Island in the Biscoe Islands.</obo:IAO_0000115>
        <oboInOwl:hasOBONamespace>GAZ</oboInOwl:hasOBONamespace>
        <oboInOwl:id>GAZ:00141319</oboInOwl:id>
        <rdfs:label>Zubov Bay</rdfs:label>
    </owl:NamedIndividual>
    


    <!-- http://purl.obolibrary.org/obo/GAZ_00141320 -->

    <owl:NamedIndividual rdf:about="http://purl.obolibrary.org/obo/GAZ_00141320">
        <obo:RO_0001025 rdf:resource="http://purl.obolibrary.org/obo/GAZ_00007425"/>
        <obo:IAO_0000115>An axial, main ice dome of King George Island.</obo:IAO_0000115>
        <oboInOwl:hasOBONamespace>GAZ</oboInOwl:hasOBONamespace>
        <oboInOwl:id>GAZ:00141320</oboInOwl:id>
        <rdfs:label>Arctowski Dome</rdfs:label>
    </owl:NamedIndividual>
    


    <!-- http://purl.obolibrary.org/obo/GAZ_00141325 -->

    <owl:NamedIndividual rdf:about="http://purl.obolibrary.org/obo/GAZ_00141325">
        <obo:RO_0001025 rdf:resource="http://purl.obolibrary.org/obo/GAZ_00139463"/>
        <obo:IAO_0000115>An ice stream flowing north into Ronne Ice Shelf, southeast of Hercules Inlet.</obo:IAO_0000115>
        <oboInOwl:hasOBONamespace>GAZ</oboInOwl:hasOBONamespace>
        <oboInOwl:id>GAZ:00141325</oboInOwl:id>
        <rdfs:label>Institute Ice Stream</rdfs:label>
    </owl:NamedIndividual>
    


    <!-- http://purl.obolibrary.org/obo/GAZ_00141326 -->

    <owl:NamedIndividual rdf:about="http://purl.obolibrary.org/obo/GAZ_00141326">
        <obo:RO_0001025 rdf:resource="http://purl.obolibrary.org/obo/GAZ_00139463"/>
        <obo:IAO_0000115>A large, narrow, ice-filled inlet which forms a part of the SW margin of Ronne Ice Shelf. It is bounded on the W by the SE flank of the Heritage Range, and on the N by Skytrain Ice Rise.</obo:IAO_0000115>
        <oboInOwl:hasOBONamespace>GAZ</oboInOwl:hasOBONamespace>
        <oboInOwl:id>GAZ:00141326</oboInOwl:id>
        <rdfs:label>Hercules Inlet</rdfs:label>
    </owl:NamedIndividual>
    


    <!-- http://purl.obolibrary.org/obo/GAZ_00141329 -->

    <owl:NamedIndividual rdf:about="http://purl.obolibrary.org/obo/GAZ_00141329">
        <obo:RO_0001025 rdf:resource="http://purl.obolibrary.org/obo/GAZ_00139463"/>
        <obo:IAO_0000115>A very large Antarctic ice rise between Evans Ice Stream and Carlson Inlet, in the southwest part of Ronne Ice Shelf.</obo:IAO_0000115>
        <oboInOwl:hasOBONamespace>GAZ</oboInOwl:hasOBONamespace>
        <oboInOwl:id>GAZ:00141329</oboInOwl:id>
        <rdfs:label>Fowler Ice Rise</rdfs:label>
    </owl:NamedIndividual>
    


    <!-- http://purl.obolibrary.org/obo/GAZ_00141330 -->

    <owl:NamedIndividual rdf:about="http://purl.obolibrary.org/obo/GAZ_00141330">
        <obo:RO_0001025 rdf:resource="http://purl.obolibrary.org/obo/GAZ_00139463"/>
        <obo:IAO_0000115>An ice-filled inlet, 100 miles long and 25 miles wide, lying between Fletcher Ice Rise and Fowler Ice Rise in the southwest part of Ronne Ice Shelf.</obo:IAO_0000115>
        <oboInOwl:hasOBONamespace>GAZ</oboInOwl:hasOBONamespace>
        <oboInOwl:id>GAZ:00141330</oboInOwl:id>
        <rdfs:label>Carlson Inlet</rdfs:label>
    </owl:NamedIndividual>
    


    <!-- http://purl.obolibrary.org/obo/GAZ_00141335 -->

    <owl:NamedIndividual rdf:about="http://purl.obolibrary.org/obo/GAZ_00141335">
        <obo:RO_0001025 rdf:resource="http://purl.obolibrary.org/obo/GAZ_00011769"/>
        <obo:IAO_0000115>An Antarctic ice rise in the south-central part of the Ross Ice Shelf.</obo:IAO_0000115>
        <oboInOwl:hasOBONamespace>GAZ</oboInOwl:hasOBONamespace>
        <oboInOwl:id>GAZ:00141335</oboInOwl:id>
        <rdfs:label>Crary Ice Rise</rdfs:label>
    </owl:NamedIndividual>
    


    <!-- http://purl.obolibrary.org/obo/GAZ_00141336 -->

    <owl:NamedIndividual rdf:about="http://purl.obolibrary.org/obo/GAZ_00141336">
        <obo:RO_0001025 rdf:resource="http://purl.obolibrary.org/obo/GAZ_00141554"/>
        <obo:IAO_0000115>The ice shelf lying between Sorasen Ridge and Halvfarryggen Ridge, on Princess Martha Coast of Queen Maud Land.</obo:IAO_0000115>
        <oboInOwl:hasOBONamespace>GAZ</oboInOwl:hasOBONamespace>
        <oboInOwl:id>GAZ:00141336</oboInOwl:id>
        <rdfs:label>Ekstrom Ice Shelf</rdfs:label>
    </owl:NamedIndividual>
    


    <!-- http://purl.obolibrary.org/obo/GAZ_00141339 -->

    <owl:NamedIndividual rdf:about="http://purl.obolibrary.org/obo/GAZ_00141339">
        <obo:RO_0001025 rdf:resource="http://purl.obolibrary.org/obo/GAZ_00141554"/>
        <obo:IAO_0000115>The ice shelf between Cape Norvegia and Sorasen Ridge along the coast of Queen Maud Land.</obo:IAO_0000115>
        <oboInOwl:hasOBONamespace>GAZ</oboInOwl:hasOBONamespace>
        <oboInOwl:id>GAZ:00141339</oboInOwl:id>
        <rdfs:label>Quar Ice Shelf</rdfs:label>
    </owl:NamedIndividual>
    


    <!-- http://purl.obolibrary.org/obo/GAZ_00141340 -->

    <owl:NamedIndividual rdf:about="http://purl.obolibrary.org/obo/GAZ_00141340">
        <obo:RO_0001025 rdf:resource="http://purl.obolibrary.org/obo/GAZ_00014090"/>
        <obo:IAO_0000115>An extensive ice shelf that occupies George VI Sound between Alexander Island and Palmer Land in Antarctica. The ice shelf extends from Ronne Entrance, at the southwest end of the sound, to Niznik Island, about 60 km south of the north entrance between Cape Brown and Cape Jeremy.</obo:IAO_0000115>
        <oboInOwl:hasOBONamespace>GAZ</oboInOwl:hasOBONamespace>
        <oboInOwl:id>GAZ:00141340</oboInOwl:id>
        <rdfs:label>George VI Ice Shelf</rdfs:label>
    </owl:NamedIndividual>
    


    <!-- http://purl.obolibrary.org/obo/GAZ_00141341 -->

    <owl:NamedIndividual rdf:about="http://purl.obolibrary.org/obo/GAZ_00141341">
        <obo:RO_0001025 rdf:resource="http://purl.obolibrary.org/obo/GAZ_00014090"/>
        <obo:IAO_0000115>An island in the N part of George VI Sound, lying opposite the mouth of Eureka Glacier near the coast of Palmer Land.</obo:IAO_0000115>
        <oboInOwl:hasOBONamespace>GAZ</oboInOwl:hasOBONamespace>
        <oboInOwl:id>GAZ:00141341</oboInOwl:id>
        <rdfs:label>Niznik Island</rdfs:label>
    </owl:NamedIndividual>
    


    <!-- http://purl.obolibrary.org/obo/GAZ_00141342 -->

    <owl:NamedIndividual rdf:about="http://purl.obolibrary.org/obo/GAZ_00141342">
        <obo:RO_0001025 rdf:resource="http://purl.obolibrary.org/obo/GAZ_00139474"/>
        <obo:IAO_0000115>The largest of the Eklund Islands.</obo:IAO_0000115>
        <oboInOwl:hasOBONamespace>GAZ</oboInOwl:hasOBONamespace>
        <oboInOwl:id>GAZ:00141342</oboInOwl:id>
        <rdfs:label>Eklund Island</rdfs:label>
    </owl:NamedIndividual>
    


    <!-- http://purl.obolibrary.org/obo/GAZ_00141343 -->

    <owl:NamedIndividual rdf:about="http://purl.obolibrary.org/obo/GAZ_00141343">
        <obo:RO_0001025 rdf:resource="http://purl.obolibrary.org/obo/GAZ_00139463"/>
        <obo:IAO_0000115>An ice rise 18 km long and 2 to 4 km wide, with an estimated area of 55 km2, located 17 km off the northwest corner of Berkner Island in Ronne Ice Shelf.</obo:IAO_0000115>
        <oboInOwl:hasOBONamespace>GAZ</oboInOwl:hasOBONamespace>
        <oboInOwl:id>GAZ:00141343</oboInOwl:id>
        <rdfs:label>Hemmen Ice Rise</rdfs:label>
    </owl:NamedIndividual>
    


    <!-- http://purl.obolibrary.org/obo/GAZ_00141344 -->

    <owl:NamedIndividual rdf:about="http://purl.obolibrary.org/obo/GAZ_00141344">
        <obo:RO_0001025 rdf:resource="http://purl.obolibrary.org/obo/GAZ_00139463"/>
        <obo:IAO_0000115>A triangular-shaped ice rise about 110 km long located between Korff Ice Rise and the southern portion of Berkner Island in the Ronne Ice Shelf.</obo:IAO_0000115>
        <oboInOwl:hasOBONamespace>GAZ</oboInOwl:hasOBONamespace>
        <oboInOwl:id>GAZ:00141344</oboInOwl:id>
        <rdfs:label>Henry Ice Rise</rdfs:label>
    </owl:NamedIndividual>
    


    <!-- http://purl.obolibrary.org/obo/GAZ_00141345 -->

    <owl:NamedIndividual rdf:about="http://purl.obolibrary.org/obo/GAZ_00141345">
        <obo:RO_0001025 rdf:resource="http://purl.obolibrary.org/obo/GAZ_00139463"/>
        <obo:IAO_0000115>An ice rise, 80 miles long and 20 miles wide, lying 50 miles eastnortheast of Skytrain Ice Rise in the southwest part of Ronne Ice Shelf.</obo:IAO_0000115>
        <oboInOwl:hasOBONamespace>GAZ</oboInOwl:hasOBONamespace>
        <oboInOwl:id>GAZ:00141345</oboInOwl:id>
        <rdfs:label>Korff Ice Rise</rdfs:label>
    </owl:NamedIndividual>
    


    <!-- http://purl.obolibrary.org/obo/GAZ_00141346 -->

    <owl:NamedIndividual rdf:about="http://purl.obolibrary.org/obo/GAZ_00141346">
        <obo:RO_0001025 rdf:resource="http://purl.obolibrary.org/obo/GAZ_00139463"/>
        <obo:IAO_0000115>A large, flattish, peninsula-like ice rise of about 50 miles extent, extending from the vicinity of Meyer Hills in the Heritage Range eastward into the Ronne Ice Shelf.</obo:IAO_0000115>
        <oboInOwl:hasOBONamespace>GAZ</oboInOwl:hasOBONamespace>
        <oboInOwl:id>GAZ:00141346</oboInOwl:id>
        <rdfs:label>Skytrain Ice Rise</rdfs:label>
    </owl:NamedIndividual>
    


    <!-- http://purl.obolibrary.org/obo/GAZ_00141347 -->

    <owl:NamedIndividual rdf:about="http://purl.obolibrary.org/obo/GAZ_00141347">
        <obo:RO_0001025 rdf:resource="http://purl.obolibrary.org/obo/GAZ_00014084"/>
        <obo:IAO_0000115>A broad ice-filled inlet, which indents the south part of Beethoven Peninsula, southwest of Bennett Dome, forming the northwest arm of Bach Ice Shelf in Alexander Island.</obo:IAO_0000115>
        <oboInOwl:hasOBONamespace>GAZ</oboInOwl:hasOBONamespace>
        <oboInOwl:id>GAZ:00141347</oboInOwl:id>
        <rdfs:label>Weber Inlet</rdfs:label>
    </owl:NamedIndividual>
    


    <!-- http://purl.obolibrary.org/obo/GAZ_00141348 -->

    <owl:NamedIndividual rdf:about="http://purl.obolibrary.org/obo/GAZ_00141348">
        <obo:RO_0001025 rdf:resource="http://purl.obolibrary.org/obo/GAZ_00141347"/>
        <obo:IAO_0000115>An ice rise about 1.6 km long at the head of Weber Inlet, southwest Alexander Island.</obo:IAO_0000115>
        <oboInOwl:hasOBONamespace>GAZ</oboInOwl:hasOBONamespace>
        <oboInOwl:id>GAZ:00141348</oboInOwl:id>
        <rdfs:label>Ives Ice Rise</rdfs:label>
    </owl:NamedIndividual>
    


    <!-- http://purl.obolibrary.org/obo/GAZ_00141349 -->

    <owl:NamedIndividual rdf:about="http://purl.obolibrary.org/obo/GAZ_00141349">
        <obo:RO_0001025 rdf:resource="http://purl.obolibrary.org/obo/GAZ_00141554"/>
        <obo:IAO_0000115>An indentation in the ice shelf fringing Queen Maud Land immediately W of Lazarev Ice Shelf.</obo:IAO_0000115>
        <oboInOwl:hasOBONamespace>GAZ</oboInOwl:hasOBONamespace>
        <oboInOwl:id>GAZ:00141349</oboInOwl:id>
        <rdfs:label>Leningradskiy Bay</rdfs:label>
    </owl:NamedIndividual>
    


    <!-- http://purl.obolibrary.org/obo/GAZ_00141350 -->

    <owl:NamedIndividual rdf:about="http://purl.obolibrary.org/obo/GAZ_00141350">
        <obo:RO_0001025 rdf:resource="http://purl.obolibrary.org/obo/GAZ_00141349"/>
        <obo:IAO_0000115>An ice-covered island situated at the head of Leningradskiy Bay at the W margin of the Lazarev Ice Shelf, Queen Maud Land.</obo:IAO_0000115>
        <oboInOwl:hasOBONamespace>GAZ</oboInOwl:hasOBONamespace>
        <oboInOwl:id>GAZ:00141350</oboInOwl:id>
        <rdfs:label>Leningradskiy Island</rdfs:label>
    </owl:NamedIndividual>
    


    <!-- http://purl.obolibrary.org/obo/GAZ_00141351 -->

    <owl:NamedIndividual rdf:about="http://purl.obolibrary.org/obo/GAZ_00141351">
        <obo:RO_0001025 rdf:resource="http://purl.obolibrary.org/obo/GAZ_00141554"/>
        <obo:IAO_0000115>That part of the ice shelf fringing the coast of Queen Maud Land between Leningradskiy Island and Verblyud Island. It is about 90 km long.</obo:IAO_0000115>
        <oboInOwl:hasOBONamespace>GAZ</oboInOwl:hasOBONamespace>
        <oboInOwl:id>GAZ:00141351</oboInOwl:id>
        <rdfs:label>Lazarev Ice Shelf</rdfs:label>
    </owl:NamedIndividual>
    


    <!-- http://purl.obolibrary.org/obo/GAZ_00141352 -->

    <owl:NamedIndividual rdf:about="http://purl.obolibrary.org/obo/GAZ_00141352">
        <obo:RO_0001025 rdf:resource="http://purl.obolibrary.org/obo/GAZ_00141554"/>
        <obo:IAO_0000115>An ice-covered island whose summit rises 200 m above the surrounding ice shelf, situated at the E margin of Lazarev Ice Shelf along the coast of Queen Maud Land.</obo:IAO_0000115>
        <oboInOwl:hasOBONamespace>GAZ</oboInOwl:hasOBONamespace>
        <oboInOwl:id>GAZ:00141352</oboInOwl:id>
        <rdfs:label>Verblyud Island</rdfs:label>
    </owl:NamedIndividual>
    


    <!-- http://purl.obolibrary.org/obo/GAZ_00141353 -->

    <owl:NamedIndividual rdf:about="http://purl.obolibrary.org/obo/GAZ_00141353">
        <obo:RO_0001025 rdf:resource="http://purl.obolibrary.org/obo/GAZ_00139225"/>
        <obo:IAO_0000115>An ice rise on the Brunt Ice Shelf bordering the Weddell Sea in Antarctica. It covers an area of 3 by 2 miles.</obo:IAO_0000115>
        <oboInOwl:hasOBONamespace>GAZ</oboInOwl:hasOBONamespace>
        <oboInOwl:id>GAZ:00141353</oboInOwl:id>
        <rdfs:label>McDonald Ice Rumples</rdfs:label>
    </owl:NamedIndividual>
    


    <!-- http://purl.obolibrary.org/obo/GAZ_00141354 -->

    <owl:NamedIndividual rdf:about="http://purl.obolibrary.org/obo/GAZ_00141354">
        <obo:RO_0001025 rdf:resource="http://purl.obolibrary.org/obo/GAZ_00139449"/>
        <obo:IAO_0000115>An ice shelf lying SW of Hooke Point in SW Lallemand Fjord, Arrowsmith Peninsula, Loubet Coast. The ice shelf is nurtured by Bruckner Glacier and Antevs Glacier.</obo:IAO_0000115>
        <oboInOwl:hasOBONamespace>GAZ</oboInOwl:hasOBONamespace>
        <oboInOwl:id>GAZ:00141354</oboInOwl:id>
        <rdfs:label>Muller Ice Shelf</rdfs:label>
    </owl:NamedIndividual>
    


    <!-- http://purl.obolibrary.org/obo/GAZ_00141359 -->

    <owl:NamedIndividual rdf:about="http://purl.obolibrary.org/obo/GAZ_00141359">
        <obo:RO_0001025 rdf:resource="http://purl.obolibrary.org/obo/GAZ_00140090"/>
        <obo:IAO_0000115>An ice shelf of more than 28 km extent occupying the south part of Prince Gustav Channel, including Rohss Bay, James Ross Island.</obo:IAO_0000115>
        <oboInOwl:hasOBONamespace>GAZ</oboInOwl:hasOBONamespace>
        <oboInOwl:id>GAZ:00141359</oboInOwl:id>
        <rdfs:label>Prince Gustav Ice Shelf</rdfs:label>
    </owl:NamedIndividual>
    


    <!-- http://purl.obolibrary.org/obo/GAZ_00141360 -->

    <owl:NamedIndividual rdf:about="http://purl.obolibrary.org/obo/GAZ_00141360">
        <obo:RO_0001025 rdf:resource="http://purl.obolibrary.org/obo/GAZ_00004045"/>
        <obo:IAO_0000115>An ice-filled inlet, 40 km long in a NW-SE direction, lying east of Churchill Peninsula along the east coast of Graham Land.</obo:IAO_0000115>
        <oboInOwl:hasOBONamespace>GAZ</oboInOwl:hasOBONamespace>
        <oboInOwl:id>GAZ:00141360</oboInOwl:id>
        <rdfs:label>Adie Inlet</rdfs:label>
    </owl:NamedIndividual>
    


    <!-- http://purl.obolibrary.org/obo/GAZ_00141361 -->

    <owl:NamedIndividual rdf:about="http://purl.obolibrary.org/obo/GAZ_00141361">
        <obo:RO_0001025 rdf:resource="http://purl.obolibrary.org/obo/GAZ_00004045"/>
        <obo:IAO_0000115>An ice-filled inlet 9 miles long, between Cape Howard and Cape MacDonald along the east coast of Palmer Land.</obo:IAO_0000115>
        <oboInOwl:hasOBONamespace>GAZ</oboInOwl:hasOBONamespace>
        <oboInOwl:id>GAZ:00141361</oboInOwl:id>
        <rdfs:label>Odom Inlet</rdfs:label>
    </owl:NamedIndividual>
    


    <!-- http://purl.obolibrary.org/obo/GAZ_00141365 -->

    <owl:NamedIndividual rdf:about="http://purl.obolibrary.org/obo/GAZ_00141365">
        <rdf:type rdf:resource="http://purl.obolibrary.org/obo/ENVO_00000100"/>
        <obo:RO_0001025 rdf:resource="http://purl.obolibrary.org/obo/GAZ_00023304"/>
        <obo:IAO_0000115>A re-entrant in the south side of Edward VII Peninsula, at the northeast corner of the Ross Ice Shelf.</obo:IAO_0000115>
        <oboInOwl:hasOBONamespace>GAZ</oboInOwl:hasOBONamespace>
        <oboInOwl:id>GAZ:00141365</oboInOwl:id>
        <rdfs:label>Prestrud Inlet</rdfs:label>
    </owl:NamedIndividual>
    


    <!-- http://purl.obolibrary.org/obo/GAZ_00141366 -->

    <owl:NamedIndividual rdf:about="http://purl.obolibrary.org/obo/GAZ_00141366">
        <obo:RO_0001025 rdf:resource="http://purl.obolibrary.org/obo/GAZ_00023304"/>
        <obo:IAO_0000115>A reentrant, about 16 km wide, between Cape Wilson and Cape Lyttelton.</obo:IAO_0000115>
        <oboInOwl:hasOBONamespace>GAZ</oboInOwl:hasOBONamespace>
        <oboInOwl:id>GAZ:00141366</oboInOwl:id>
        <rdfs:label>Shackleton Inlet</rdfs:label>
    </owl:NamedIndividual>
    


    <!-- http://purl.obolibrary.org/obo/GAZ_00141394 -->

    <owl:NamedIndividual rdf:about="http://purl.obolibrary.org/obo/GAZ_00141394">
        <obo:RO_0001025 rdf:resource="http://purl.obolibrary.org/obo/GAZ_00004057"/>
        <obo:IAO_0000115>A lake lying southeast of Skua Lake at Cape Evans, Ross Island.</obo:IAO_0000115>
        <oboInOwl:hasOBONamespace>GAZ</oboInOwl:hasOBONamespace>
        <oboInOwl:id>GAZ:00141394</oboInOwl:id>
        <rdfs:label>Island Lake</rdfs:label>
    </owl:NamedIndividual>
    


    <!-- http://purl.obolibrary.org/obo/GAZ_00141404 -->

    <owl:NamedIndividual rdf:about="http://purl.obolibrary.org/obo/GAZ_00141404">
        <obo:RO_0001025 rdf:resource="http://purl.obolibrary.org/obo/GAZ_00141275"/>
        <obo:IAO_0000115>A lake just southeast of Showa Flat in the east extremity of Ongul Island.</obo:IAO_0000115>
        <oboInOwl:hasOBONamespace>GAZ</oboInOwl:hasOBONamespace>
        <oboInOwl:id>GAZ:00141404</oboInOwl:id>
        <rdfs:label>Lake O-ike</rdfs:label>
    </owl:NamedIndividual>
    


    <!-- http://purl.obolibrary.org/obo/GAZ_00141405 -->

    <owl:NamedIndividual rdf:about="http://purl.obolibrary.org/obo/GAZ_00141405">
        <obo:RO_0001025 rdf:resource="http://purl.obolibrary.org/obo/GAZ_00141275"/>
        <obo:IAO_0000115>A small flattish area along the northwest shore of Lake O-ike in the east part of Ongul Island.</obo:IAO_0000115>
        <oboInOwl:hasOBONamespace>GAZ</oboInOwl:hasOBONamespace>
        <oboInOwl:id>GAZ:00141405</oboInOwl:id>
        <rdfs:label>Showa Flat</rdfs:label>
    </owl:NamedIndividual>
    


    <!-- http://purl.obolibrary.org/obo/GAZ_00141426 -->

    <owl:NamedIndividual rdf:about="http://purl.obolibrary.org/obo/GAZ_00141426">
        <obo:RO_0001025 rdf:resource="http://purl.obolibrary.org/obo/GAZ_00141427"/>
        <obo:IAO_0000115>The topographic feature that embraces the crater within the floor of Main Crater, at the summit of Mount Erebus, Ross Island. Inner Crater contains an active anorthoclase-phonolite lava lake.</obo:IAO_0000115>
        <oboInOwl:hasOBONamespace>GAZ</oboInOwl:hasOBONamespace>
        <oboInOwl:id>GAZ:00141426</oboInOwl:id>
        <rdfs:label>Inner Crater</rdfs:label>
    </owl:NamedIndividual>
    


    <!-- http://purl.obolibrary.org/obo/GAZ_00141427 -->

    <owl:NamedIndividual rdf:about="http://purl.obolibrary.org/obo/GAZ_00141427">
        <obo:RO_0001025 rdf:resource="http://purl.obolibrary.org/obo/GAZ_00014119"/>
        <obo:IAO_0000115>The topographic feature that rises to c.3750 m and forms the primary summit crater of Mount Erebus on Ross Island.</obo:IAO_0000115>
        <oboInOwl:hasOBONamespace>GAZ</oboInOwl:hasOBONamespace>
        <oboInOwl:id>GAZ:00141427</oboInOwl:id>
        <rdfs:label>Main Crater</rdfs:label>
    </owl:NamedIndividual>
    


    <!-- http://purl.obolibrary.org/obo/GAZ_00141428 -->

    <owl:NamedIndividual rdf:about="http://purl.obolibrary.org/obo/GAZ_00141428">
        <obo:RO_0001025 rdf:resource="http://purl.obolibrary.org/obo/GAZ_00045047"/>
        <obo:IAO_0000115>A caldera on Coulman Island.</obo:IAO_0000115>
        <oboInOwl:hasOBONamespace>GAZ</oboInOwl:hasOBONamespace>
        <oboInOwl:id>GAZ:00141428</oboInOwl:id>
        <rdfs:label>Coulman Caldera</rdfs:label>
    </owl:NamedIndividual>
    


    <!-- http://purl.obolibrary.org/obo/GAZ_00141455 -->

    <owl:NamedIndividual rdf:about="http://purl.obolibrary.org/obo/GAZ_00141455">
        <obo:RO_0001025 rdf:resource="http://purl.obolibrary.org/obo/GAZ_00007425"/>
        <obo:IAO_0000115>A small valley lying east-northeast of Herve Cove, Ezcurra Inlet, King George Island, in the South Shetland Islands.</obo:IAO_0000115>
        <oboInOwl:hasOBONamespace>GAZ</oboInOwl:hasOBONamespace>
        <oboInOwl:id>GAZ:00141455</oboInOwl:id>
        <rdfs:label>Italia Valley</rdfs:label>
    </owl:NamedIndividual>
    


    <!-- http://purl.obolibrary.org/obo/GAZ_00141456 -->

    <owl:NamedIndividual rdf:about="http://purl.obolibrary.org/obo/GAZ_00141456">
        <obo:RO_0001025 rdf:resource="http://purl.obolibrary.org/obo/GAZ_00139126"/>
        <obo:IAO_0000115>A small cove 2 mi SW of Point Thomas, along the S side of Ezcurra Inlet, Admiralty Bay, on King George Island in the South Shetland Islands.</obo:IAO_0000115>
        <oboInOwl:hasOBONamespace>GAZ</oboInOwl:hasOBONamespace>
        <oboInOwl:id>GAZ:00141456</oboInOwl:id>
        <rdfs:label>Herve Cove</rdfs:label>
    </owl:NamedIndividual>
    


    <!-- http://purl.obolibrary.org/obo/GAZ_00141463 -->

    <owl:NamedIndividual rdf:about="http://purl.obolibrary.org/obo/GAZ_00141463">
        <obo:RO_0001025 rdf:resource="http://purl.obolibrary.org/obo/GAZ_00045077"/>
        <obo:IAO_0000115>A small valley trending NE-SW, located 1.6 km east-southeast of Stoneley Point on James Ross Island.</obo:IAO_0000115>
        <oboInOwl:hasOBONamespace>GAZ</oboInOwl:hasOBONamespace>
        <oboInOwl:id>GAZ:00141463</oboInOwl:id>
        <rdfs:label>Sharp Valley</rdfs:label>
    </owl:NamedIndividual>
    


    <!-- http://purl.obolibrary.org/obo/GAZ_00141464 -->

    <owl:NamedIndividual rdf:about="http://purl.obolibrary.org/obo/GAZ_00141464">
        <obo:RO_0001025 rdf:resource="http://purl.obolibrary.org/obo/GAZ_00045077"/>
        <obo:IAO_0000115>A rocky point on the NW coast of James Ross Island, 4 mi W of Brandy Bay.</obo:IAO_0000115>
        <oboInOwl:hasOBONamespace>GAZ</oboInOwl:hasOBONamespace>
        <oboInOwl:id>GAZ:00141464</oboInOwl:id>
        <rdfs:label>Stoneley Point</rdfs:label>
    </owl:NamedIndividual>
    


    <!-- http://purl.obolibrary.org/obo/GAZ_00141465 -->

    <owl:NamedIndividual rdf:about="http://purl.obolibrary.org/obo/GAZ_00141465">
        <obo:RO_0001025 rdf:resource="http://purl.obolibrary.org/obo/GAZ_00004045"/>
        <obo:IAO_0000115>A bay 2 mi wide on the NW coast of James Ross Island, entered W of Bibby Point.</obo:IAO_0000115>
        <oboInOwl:hasOBONamespace>GAZ</oboInOwl:hasOBONamespace>
        <oboInOwl:id>GAZ:00141465</oboInOwl:id>
        <rdfs:label>Brandy Bay</rdfs:label>
    </owl:NamedIndividual>
    


    <!-- http://purl.obolibrary.org/obo/GAZ_00141466 -->

    <owl:NamedIndividual rdf:about="http://purl.obolibrary.org/obo/GAZ_00141466">
        <obo:RO_0001025 rdf:resource="http://purl.obolibrary.org/obo/GAZ_00045077"/>
        <obo:IAO_0000115>A steep rocky point with snow slopes falling away inland, at the NE corner of Brandy Bay, James Ross Island.</obo:IAO_0000115>
        <oboInOwl:hasOBONamespace>GAZ</oboInOwl:hasOBONamespace>
        <oboInOwl:id>GAZ:00141466</oboInOwl:id>
        <rdfs:label>Bibby Point</rdfs:label>
    </owl:NamedIndividual>
    


    <!-- http://purl.obolibrary.org/obo/GAZ_00141467 -->

    <owl:NamedIndividual rdf:about="http://purl.obolibrary.org/obo/GAZ_00141467">
        <obo:RO_0001025 rdf:resource="http://purl.obolibrary.org/obo/GAZ_00141023"/>
        <obo:IAO_0000115>An undersea valley named in association with the Vanderford Glacier. This may be the deepest glacier-carved valley in the world.</obo:IAO_0000115>
        <oboInOwl:hasOBONamespace>GAZ</oboInOwl:hasOBONamespace>
        <oboInOwl:id>GAZ:00141467</oboInOwl:id>
        <rdfs:label>Vanderford Valley</rdfs:label>
    </owl:NamedIndividual>
    


    <!-- http://purl.obolibrary.org/obo/GAZ_00141468 -->

    <owl:NamedIndividual rdf:about="http://purl.obolibrary.org/obo/GAZ_00141468">
        <obo:RO_0001025 rdf:resource="http://purl.obolibrary.org/obo/GAZ_00141552"/>
        <obo:IAO_0000115>A marine channel between Lemaire Island and Danco Coast, permitting northern access to Paradise Harbor.</obo:IAO_0000115>
        <oboInOwl:hasOBONamespace>GAZ</oboInOwl:hasOBONamespace>
        <oboInOwl:id>GAZ:00141468</oboInOwl:id>
        <rdfs:label>Aguirre Passage</rdfs:label>
    </owl:NamedIndividual>
    


    <!-- http://purl.obolibrary.org/obo/GAZ_00141469 -->

    <owl:NamedIndividual rdf:about="http://purl.obolibrary.org/obo/GAZ_00141469">
        <obo:RO_0001025 rdf:resource="http://purl.obolibrary.org/obo/GAZ_00141552"/>
        <obo:IAO_0000115>An island 4.5 mi long and 1.5 mi wide, lying 1 mi W of Duthiers Point off the W coast of Graham Land.</obo:IAO_0000115>
        <oboInOwl:hasOBONamespace>GAZ</oboInOwl:hasOBONamespace>
        <oboInOwl:id>GAZ:00141469</oboInOwl:id>
        <rdfs:label>Lemaire Island</rdfs:label>
    </owl:NamedIndividual>
    


    <!-- http://purl.obolibrary.org/obo/GAZ_00141470 -->

    <owl:NamedIndividual rdf:about="http://purl.obolibrary.org/obo/GAZ_00141470">
        <obo:RO_0001025 rdf:resource="http://purl.obolibrary.org/obo/GAZ_00023348"/>
        <obo:IAO_0000115>An undersea trough under Bransfield Strait.</obo:IAO_0000115>
        <oboInOwl:hasOBONamespace>GAZ</oboInOwl:hasOBONamespace>
        <oboInOwl:id>GAZ:00141470</oboInOwl:id>
        <rdfs:label>Bransfield Trough</rdfs:label>
    </owl:NamedIndividual>
    


    <!-- http://purl.obolibrary.org/obo/GAZ_00141471 -->

    <owl:NamedIndividual rdf:about="http://purl.obolibrary.org/obo/GAZ_00141471">
        <obo:RO_0001025 rdf:resource="http://purl.obolibrary.org/obo/GAZ_00014084"/>
        <obo:IAO_0000115>A marine channel in Hanusse Bay between Liard Island and Arrowsmith Peninsula on the west coast of Graham Land.</obo:IAO_0000115>
        <oboInOwl:hasOBONamespace>GAZ</oboInOwl:hasOBONamespace>
        <oboInOwl:id>GAZ:00141471</oboInOwl:id>
        <rdfs:label>Isacke Passage</rdfs:label>
    </owl:NamedIndividual>
    


    <!-- http://purl.obolibrary.org/obo/GAZ_00141472 -->

    <owl:NamedIndividual rdf:about="http://purl.obolibrary.org/obo/GAZ_00141472">
        <obo:RO_0001025 rdf:resource="http://purl.obolibrary.org/obo/GAZ_00004045"/>
        <obo:IAO_0000115>A strait 1 to 3 miles wide between D&apos;Urville Island and Joinville Island, off the northeastern end of the Antarctic Peninsula.</obo:IAO_0000115>
        <oboInOwl:hasOBONamespace>GAZ</oboInOwl:hasOBONamespace>
        <oboInOwl:id>GAZ:00141472</oboInOwl:id>
        <rdfs:label>Larsen Channel</rdfs:label>
    </owl:NamedIndividual>
    


    <!-- http://purl.obolibrary.org/obo/GAZ_00141473 -->

    <owl:NamedIndividual rdf:about="http://purl.obolibrary.org/obo/GAZ_00141473">
        <obo:RO_0001025 rdf:resource="http://purl.obolibrary.org/obo/GAZ_00141552"/>
        <obo:IAO_0000115>A strait off Antarctica, located between the mainland&apos;s Antarctic Peninsula and Booth Island.</obo:IAO_0000115>
        <oboInOwl:hasOBONamespace>GAZ</oboInOwl:hasOBONamespace>
        <oboInOwl:id>GAZ:00141473</oboInOwl:id>
        <rdfs:label>Lemaire Channel</rdfs:label>
    </owl:NamedIndividual>
    


    <!-- http://purl.obolibrary.org/obo/GAZ_00141474 -->

    <owl:NamedIndividual rdf:about="http://purl.obolibrary.org/obo/GAZ_00141474">
        <obo:RO_0001025 rdf:resource="http://purl.obolibrary.org/obo/GAZ_00051518"/>
        <obo:IAO_0000115>A narrow island 0.5 mi long with a serrated coastline, lying 0.1 mi N of Galindez Island in the Argentine Islands, Wilhelm Archipelago.</obo:IAO_0000115>
        <oboInOwl:hasOBONamespace>GAZ</oboInOwl:hasOBONamespace>
        <oboInOwl:id>GAZ:00141474</oboInOwl:id>
        <rdfs:label>Grotto Island</rdfs:label>
    </owl:NamedIndividual>
    


    <!-- http://purl.obolibrary.org/obo/GAZ_00141475 -->

    <owl:NamedIndividual rdf:about="http://purl.obolibrary.org/obo/GAZ_00141475">
        <obo:RO_0001025 rdf:resource="http://purl.obolibrary.org/obo/GAZ_00051518"/>
        <obo:IAO_0000115>A small island in the form of a crude right angle, lying 0.1 mi NE of Galindez Island in the Argentine Islands, Wilhelm Archipelago.</obo:IAO_0000115>
        <oboInOwl:hasOBONamespace>GAZ</oboInOwl:hasOBONamespace>
        <oboInOwl:id>GAZ:00141475</oboInOwl:id>
        <rdfs:label>Corner Island</rdfs:label>
    </owl:NamedIndividual>
    


    <!-- http://purl.obolibrary.org/obo/GAZ_00141476 -->

    <owl:NamedIndividual rdf:about="http://purl.obolibrary.org/obo/GAZ_00141476">
        <obo:RO_0001025 rdf:resource="http://purl.obolibrary.org/obo/GAZ_00141552"/>
        <obo:IAO_0000115>A narrow channel separating Galindez Island from Grotto Island and Corner Island in the Argentine Islands, Wilhelm Archipelago.</obo:IAO_0000115>
        <oboInOwl:hasOBONamespace>GAZ</oboInOwl:hasOBONamespace>
        <oboInOwl:id>GAZ:00141476</oboInOwl:id>
        <rdfs:label>Meek Channel</rdfs:label>
    </owl:NamedIndividual>
    


    <!-- http://purl.obolibrary.org/obo/GAZ_00141477 -->

    <owl:NamedIndividual rdf:about="http://purl.obolibrary.org/obo/GAZ_00141477">
        <obo:RO_0001025 rdf:resource="http://purl.obolibrary.org/obo/GAZ_00141552"/>
        <obo:IAO_0000115>A channel 26 km long in a NE-SW direction and about 2.4 km wide, separating Anvers Island from Wiencke Island and Doumer Island, in the Palmer Archipelago.</obo:IAO_0000115>
        <oboInOwl:hasOBONamespace>GAZ</oboInOwl:hasOBONamespace>
        <oboInOwl:id>GAZ:00141477</oboInOwl:id>
        <rdfs:label>Neumayer Channel</rdfs:label>
    </owl:NamedIndividual>
    


    <!-- http://purl.obolibrary.org/obo/GAZ_00141478 -->

    <owl:NamedIndividual rdf:about="http://purl.obolibrary.org/obo/GAZ_00141478">
        <obo:RO_0001025 rdf:resource="http://purl.obolibrary.org/obo/GAZ_00140059"/>
        <obo:IAO_0000115>A strait 9 km wide between Cornwallis and Elephant Islands, in the South Shetland Islands.</obo:IAO_0000115>
        <oboInOwl:hasOBONamespace>GAZ</oboInOwl:hasOBONamespace>
        <oboInOwl:id>GAZ:00141478</oboInOwl:id>
        <rdfs:label>Prince Charles Strait</rdfs:label>
    </owl:NamedIndividual>
    


    <!-- http://purl.obolibrary.org/obo/GAZ_00141479 -->

    <owl:NamedIndividual rdf:about="http://purl.obolibrary.org/obo/GAZ_00141479">
        <obo:RO_0001025 rdf:resource="http://purl.obolibrary.org/obo/GAZ_00014089"/>
        <obo:IAO_0000115>A channel leading southwestward from Adelaide Anchorage between Hibbert Rock and Henkes Islands, off the south end of Adelaide Island.</obo:IAO_0000115>
        <oboInOwl:hasOBONamespace>GAZ</oboInOwl:hasOBONamespace>
        <oboInOwl:id>GAZ:00141479</oboInOwl:id>
        <rdfs:label>Quest Channel</rdfs:label>
    </owl:NamedIndividual>
    


    <!-- http://purl.obolibrary.org/obo/GAZ_00141480 -->

    <owl:NamedIndividual rdf:about="http://purl.obolibrary.org/obo/GAZ_00141480">
        <obo:RO_0001025 rdf:resource="http://purl.obolibrary.org/obo/GAZ_00004045"/>
        <obo:IAO_0000115>A sound which extends in a NE-SW direction and separates Seymour and Snow Hill Islands from James Ross Island, off the NE end of Antarctic Peninsula.</obo:IAO_0000115>
        <oboInOwl:hasOBONamespace>GAZ</oboInOwl:hasOBONamespace>
        <oboInOwl:id>GAZ:00141480</oboInOwl:id>
        <rdfs:label>Admiralty Sound</rdfs:label>
    </owl:NamedIndividual>
    


    <!-- http://purl.obolibrary.org/obo/GAZ_00141481 -->

    <owl:NamedIndividual rdf:about="http://purl.obolibrary.org/obo/GAZ_00141481">
        <obo:RO_0001025 rdf:resource="http://purl.obolibrary.org/obo/GAZ_00014089"/>
        <obo:IAO_0000115>A drying rock lying SE of League Rock, off the S end of Adelaide Island.</obo:IAO_0000115>
        <oboInOwl:hasOBONamespace>GAZ</oboInOwl:hasOBONamespace>
        <oboInOwl:id>GAZ:00141481</oboInOwl:id>
        <rdfs:label>Hibbert Rock</rdfs:label>
    </owl:NamedIndividual>
    


    <!-- http://purl.obolibrary.org/obo/GAZ_00141482 -->

    <owl:NamedIndividual rdf:about="http://purl.obolibrary.org/obo/GAZ_00141482">
        <obo:RO_0001025 rdf:resource="http://purl.obolibrary.org/obo/GAZ_00014089"/>
        <obo:IAO_0000115>A distinctive rounded rock lying SW of Box Reef, off the S end of Adelaide Island.</obo:IAO_0000115>
        <oboInOwl:hasOBONamespace>GAZ</oboInOwl:hasOBONamespace>
        <oboInOwl:id>GAZ:00141482</oboInOwl:id>
        <rdfs:label>League Rock</rdfs:label>
    </owl:NamedIndividual>
    


    <!-- http://purl.obolibrary.org/obo/GAZ_00141483 -->

    <owl:NamedIndividual rdf:about="http://purl.obolibrary.org/obo/GAZ_00141483">
        <obo:RO_0001025 rdf:resource="http://purl.obolibrary.org/obo/GAZ_00141552"/>
        <obo:IAO_0000115>A narrow channel between Pourquoi Pas Island and Blaiklock Island, connecting Bigourdan Fjord and Bourgeois Fjord off the west coast of Graham Land.</obo:IAO_0000115>
        <oboInOwl:hasOBONamespace>GAZ</oboInOwl:hasOBONamespace>
        <oboInOwl:id>GAZ:00141483</oboInOwl:id>
        <rdfs:label>The Narrows</rdfs:label>
    </owl:NamedIndividual>
    


    <!-- http://purl.obolibrary.org/obo/GAZ_00141484 -->

    <owl:NamedIndividual rdf:about="http://purl.obolibrary.org/obo/GAZ_00141484">
        <obo:RO_0001025 rdf:resource="http://purl.obolibrary.org/obo/GAZ_00014089"/>
        <obo:IAO_0000115>A group of small islands and rocks 2 mi in extent, lying 1 mi SW of Avian Island, close off the S extremity of Adelaide Island.</obo:IAO_0000115>
        <oboInOwl:hasOBONamespace>GAZ</oboInOwl:hasOBONamespace>
        <oboInOwl:id>GAZ:00141484</oboInOwl:id>
        <rdfs:label>Henkes Islands</rdfs:label>
    </owl:NamedIndividual>
    


    <!-- http://purl.obolibrary.org/obo/GAZ_00141485 -->

    <owl:NamedIndividual rdf:about="http://purl.obolibrary.org/obo/GAZ_00141485">
        <rdf:type rdf:resource="http://purl.obolibrary.org/obo/ENVO_00000029"/>
        <obo:RO_0001025 rdf:resource="http://purl.obolibrary.org/obo/GAZ_00141024"/>
        <obo:IAO_0000115>A passage 4.8 km wide between Fredriksen and Powell Islands on the west and Laurie Island and several smaller islands on the east, in the South Orkney Islands.</obo:IAO_0000115>
        <oboInOwl:hasOBONamespace>GAZ</oboInOwl:hasOBONamespace>
        <oboInOwl:id>GAZ:00141485</oboInOwl:id>
        <rdfs:label>Washington Strait</rdfs:label>
    </owl:NamedIndividual>
    


    <!-- http://purl.obolibrary.org/obo/GAZ_00141486 -->

    <owl:NamedIndividual rdf:about="http://purl.obolibrary.org/obo/GAZ_00141486">
        <obo:RO_0001025 rdf:resource="http://purl.obolibrary.org/obo/GAZ_00004045"/>
        <obo:IAO_0000115>A sound, averaging 3.2 km wide, extending in an east-northeast direction from Antarctic Sound and joining the Firth of Tay with which it separates Joinville and Dundee Islands.</obo:IAO_0000115>
        <oboInOwl:hasOBONamespace>GAZ</oboInOwl:hasOBONamespace>
        <oboInOwl:id>GAZ:00141486</oboInOwl:id>
        <rdfs:label>Active Sound</rdfs:label>
    </owl:NamedIndividual>
    


    <!-- http://purl.obolibrary.org/obo/GAZ_00141487 -->

    <owl:NamedIndividual rdf:about="http://purl.obolibrary.org/obo/GAZ_00141487">
        <obo:RO_0001025 rdf:resource="http://purl.obolibrary.org/obo/GAZ_00004045"/>
        <obo:IAO_0000115>A sound, 19 km long and 10 km wide, extending in a NW-SE direction between the northeast side of Dundee Island and the east portion of Joinville Island. It merges to the northwest with Active Sound with which it completes the separation of Dundee and Joinville Islands.</obo:IAO_0000115>
        <oboInOwl:hasOBONamespace>GAZ</oboInOwl:hasOBONamespace>
        <oboInOwl:id>GAZ:00141487</oboInOwl:id>
        <rdfs:label>Firth of Tay</rdfs:label>
    </owl:NamedIndividual>
    


    <!-- http://purl.obolibrary.org/obo/GAZ_00141488 -->

    <owl:NamedIndividual rdf:about="http://purl.obolibrary.org/obo/GAZ_00141488">
        <obo:RO_0001025 rdf:resource="http://purl.obolibrary.org/obo/GAZ_00004045"/>
        <obo:IAO_0000115>A sound in Antarctica extending from Cape Lachman and Keltie Head on the northwest to the narrows between The Naze and False Island Point on the southeast, separating Vega Island from James Ross Island and connecting Prince Gustav Channel with Erebus and Terror Gulf.</obo:IAO_0000115>
        <oboInOwl:hasOBONamespace>GAZ</oboInOwl:hasOBONamespace>
        <oboInOwl:id>GAZ:00141488</oboInOwl:id>
        <rdfs:label>Herbert Sound</rdfs:label>
    </owl:NamedIndividual>
    


    <!-- http://purl.obolibrary.org/obo/GAZ_00141489 -->

    <owl:NamedIndividual rdf:about="http://purl.obolibrary.org/obo/GAZ_00141489">
        <obo:RO_0001025 rdf:resource="http://purl.obolibrary.org/obo/GAZ_00004045"/>
        <obo:IAO_0000115>A sound, 6 mi long in a N-S direction and 2 mi wide, which separates Andersson and Jonassen Islands from Tabarin Peninsula, at the NE end of Antarctic Peninsula.</obo:IAO_0000115>
        <oboInOwl:hasOBONamespace>GAZ</oboInOwl:hasOBONamespace>
        <oboInOwl:id>GAZ:00141489</oboInOwl:id>
        <rdfs:label>Fridtjof Sound</rdfs:label>
    </owl:NamedIndividual>
    


    <!-- http://purl.obolibrary.org/obo/GAZ_00141490 -->

    <owl:NamedIndividual rdf:about="http://purl.obolibrary.org/obo/GAZ_00141490">
        <rdf:type rdf:resource="http://purl.obolibrary.org/obo/ENVO_00000029"/>
        <obo:RO_0001025 rdf:resource="http://purl.obolibrary.org/obo/GAZ_00004045"/>
        <obo:IAO_0000115>A passage 1.6 km wide and 6 km long, usually ice bound, linking Fridtjof Sound and Antarctic Sound between Jonassen Island and Andersson Island, off Trinity Peninsula.</obo:IAO_0000115>
        <oboInOwl:hasOBONamespace>GAZ</oboInOwl:hasOBONamespace>
        <oboInOwl:id>GAZ:00141490</oboInOwl:id>
        <rdfs:label>Yalour Sound</rdfs:label>
    </owl:NamedIndividual>
    


    <!-- http://purl.obolibrary.org/obo/GAZ_00141491 -->

    <owl:NamedIndividual rdf:about="http://purl.obolibrary.org/obo/GAZ_00141491">
        <obo:RO_0001025 rdf:resource="http://purl.obolibrary.org/obo/GAZ_00004045"/>
        <obo:IAO_0000115>An island located at the eastern end of the Tabarin Peninsula, Antarctica.</obo:IAO_0000115>
        <oboInOwl:hasOBONamespace>GAZ</oboInOwl:hasOBONamespace>
        <oboInOwl:id>GAZ:00141491</oboInOwl:id>
        <rdfs:label>Andersson Island</rdfs:label>
    </owl:NamedIndividual>
    


    <!-- http://purl.obolibrary.org/obo/GAZ_00141493 -->

    <owl:NamedIndividual rdf:about="http://purl.obolibrary.org/obo/GAZ_00141493">
        <obo:RO_0001025 rdf:resource="http://purl.obolibrary.org/obo/GAZ_00004045"/>
        <obo:IAO_0000115>An island off the N end of the Antarctic Peninsula.</obo:IAO_0000115>
        <oboInOwl:hasOBONamespace>GAZ</oboInOwl:hasOBONamespace>
        <oboInOwl:id>GAZ:00141493</oboInOwl:id>
        <rdfs:label>Jonassen Island</rdfs:label>
    </owl:NamedIndividual>
    


    <!-- http://purl.obolibrary.org/obo/GAZ_00141494 -->

    <owl:NamedIndividual rdf:about="http://purl.obolibrary.org/obo/GAZ_00141494">
        <obo:RO_0001025 rdf:resource="http://purl.obolibrary.org/obo/GAZ_00004380"/>
        <obo:IAO_0000115>A small island close off the south coast of Tower Island, Palmer Archipelago.</obo:IAO_0000115>
        <oboInOwl:hasOBONamespace>GAZ</oboInOwl:hasOBONamespace>
        <oboInOwl:id>GAZ:00141494</oboInOwl:id>
        <rdfs:label>Zigzag Island</rdfs:label>
    </owl:NamedIndividual>
    


    <!-- http://purl.obolibrary.org/obo/GAZ_00141495 -->

    <owl:NamedIndividual rdf:about="http://purl.obolibrary.org/obo/GAZ_00141495">
        <obo:RO_0001025 rdf:resource="http://purl.obolibrary.org/obo/GAZ_00004045"/>
        <obo:IAO_0000115>An island 5 mi long and 4 mi wide, rising to 560 m on the NE side. It is the largest island in the archipelago which lies between Trinity Peninsula and Vega Island.</obo:IAO_0000115>
        <oboInOwl:hasOBONamespace>GAZ</oboInOwl:hasOBONamespace>
        <oboInOwl:id>GAZ:00141495</oboInOwl:id>
        <rdfs:label>Eagle Island</rdfs:label>
    </owl:NamedIndividual>
    


    <!-- http://purl.obolibrary.org/obo/GAZ_00141502 -->

    <owl:NamedIndividual rdf:about="http://purl.obolibrary.org/obo/GAZ_00141502">
        <obo:RO_0001025 rdf:resource="http://purl.obolibrary.org/obo/GAZ_00002625"/>
        <obo:IAO_0000115>A cove along the W margin of McMurdo Sound between Gneiss Point and Marble Point, Victoria Land.</obo:IAO_0000115>
        <oboInOwl:hasOBONamespace>GAZ</oboInOwl:hasOBONamespace>
        <oboInOwl:id>GAZ:00141502</oboInOwl:id>
        <rdfs:label>Arnold Cove</rdfs:label>
    </owl:NamedIndividual>
    


    <!-- http://purl.obolibrary.org/obo/GAZ_00141508 -->

    <owl:NamedIndividual rdf:about="http://purl.obolibrary.org/obo/GAZ_00141508">
        <obo:RO_0001025 rdf:resource="http://purl.obolibrary.org/obo/GAZ_00045024"/>
        <obo:IAO_0000115>A reef which encompasses a large number of small islands and rocks, extending 16 km southwest from the south end of Rabot Island, in the Biscoe Islands.</obo:IAO_0000115>
        <oboInOwl:hasOBONamespace>GAZ</oboInOwl:hasOBONamespace>
        <oboInOwl:id>GAZ:00141508</oboInOwl:id>
        <rdfs:label>Extension Reef</rdfs:label>
    </owl:NamedIndividual>
    


    <!-- http://purl.obolibrary.org/obo/GAZ_00141509 -->

    <owl:NamedIndividual rdf:about="http://purl.obolibrary.org/obo/GAZ_00141509">
        <obo:RO_0001025 rdf:resource="http://purl.obolibrary.org/obo/GAZ_00014089"/>
        <obo:IAO_0000115>A reef lying 13 km west of Red Rock Ridge in Marguerite Bay.</obo:IAO_0000115>
        <oboInOwl:hasOBONamespace>GAZ</oboInOwl:hasOBONamespace>
        <oboInOwl:id>GAZ:00141509</oboInOwl:id>
        <rdfs:label>Endurance Reef</rdfs:label>
    </owl:NamedIndividual>
    


    <!-- http://purl.obolibrary.org/obo/GAZ_00141510 -->

    <owl:NamedIndividual rdf:about="http://purl.obolibrary.org/obo/GAZ_00141510">
        <obo:RO_0001025 rdf:resource="http://purl.obolibrary.org/obo/GAZ_00141487"/>
        <obo:IAO_0000115>An isolated reef lying in the Firth of Tay, just off the north coast of Dundee Island.</obo:IAO_0000115>
        <oboInOwl:hasOBONamespace>GAZ</oboInOwl:hasOBONamespace>
        <oboInOwl:id>GAZ:00141510</oboInOwl:id>
        <rdfs:label>Active Reef</rdfs:label>
    </owl:NamedIndividual>
    


    <!-- http://purl.obolibrary.org/obo/GAZ_00141525 -->

    <owl:NamedIndividual rdf:about="http://purl.obolibrary.org/obo/GAZ_00141525">
        <obo:RO_0001025 rdf:resource="http://purl.obolibrary.org/obo/GAZ_00045077"/>
        <obo:IAO_0000115>A gravel plain cut by braided streams at the head of Brandy Bay, James Ross Island.</obo:IAO_0000115>
        <oboInOwl:hasOBONamespace>GAZ</oboInOwl:hasOBONamespace>
        <oboInOwl:id>GAZ:00141525</oboInOwl:id>
        <rdfs:label>Abernethy Flats</rdfs:label>
    </owl:NamedIndividual>
    


    <!-- http://purl.obolibrary.org/obo/GAZ_00141529 -->

    <owl:NamedIndividual rdf:about="http://purl.obolibrary.org/obo/GAZ_00141529">
        <obo:RO_0001025 rdf:resource="http://purl.obolibrary.org/obo/GAZ_00140059"/>
        <obo:IAO_0000115>A cove indenting the SW part of King George Island between Collins Harbor and Potter Cove, in the South Shetland Islands.</obo:IAO_0000115>
        <oboInOwl:hasOBONamespace>GAZ</oboInOwl:hasOBONamespace>
        <oboInOwl:id>GAZ:00141529</oboInOwl:id>
        <rdfs:label>Marian Cove</rdfs:label>
    </owl:NamedIndividual>
    


    <!-- http://purl.obolibrary.org/obo/GAZ_00141534 -->

    <owl:NamedIndividual rdf:about="http://purl.obolibrary.org/obo/GAZ_00141534">
        <obo:RO_0001025 rdf:resource="http://purl.obolibrary.org/obo/GAZ_00014088"/>
        <obo:IAO_0000115>An ice-covered peninsula lying north of Stravinsky Inlet and extending into Bach Ice Shelf in southern Alexander Island.</obo:IAO_0000115>
        <oboInOwl:hasOBONamespace>GAZ</oboInOwl:hasOBONamespace>
        <oboInOwl:id>GAZ:00141534</oboInOwl:id>
        <rdfs:label>Shostakovich Peninsula</rdfs:label>
    </owl:NamedIndividual>
    


    <!-- http://purl.obolibrary.org/obo/GAZ_00141535 -->

    <owl:NamedIndividual rdf:about="http://purl.obolibrary.org/obo/GAZ_00141535">
        <obo:RO_0001025 rdf:resource="http://purl.obolibrary.org/obo/GAZ_00014088"/>
        <obo:IAO_0000115>A large ice-covered peninsula between Bach Ice Shelf and George VI Sound, forming the southernmost part of Alexander Island.</obo:IAO_0000115>
        <oboInOwl:hasOBONamespace>GAZ</oboInOwl:hasOBONamespace>
        <oboInOwl:id>GAZ:00141535</oboInOwl:id>
        <rdfs:label>Monteverdi Peninsula</rdfs:label>
    </owl:NamedIndividual>
    


    <!-- http://purl.obolibrary.org/obo/GAZ_00141536 -->

    <owl:NamedIndividual rdf:about="http://purl.obolibrary.org/obo/GAZ_00141536">
        <obo:RO_0001025 rdf:resource="http://purl.obolibrary.org/obo/GAZ_00014084"/>
        <obo:IAO_0000115>An ice-covered inlet between Shostakovich Peninsula and Monteverdi Peninsula in southern Alexander Island.</obo:IAO_0000115>
        <oboInOwl:hasOBONamespace>GAZ</oboInOwl:hasOBONamespace>
        <oboInOwl:id>GAZ:00141536</oboInOwl:id>
        <rdfs:label>Stravinsky Inlet</rdfs:label>
    </owl:NamedIndividual>
    


    <!-- http://purl.obolibrary.org/obo/GAZ_00141538 -->

    <owl:NamedIndividual rdf:about="http://purl.obolibrary.org/obo/GAZ_00141538">
        <rdf:type rdf:resource="http://purl.obolibrary.org/obo/ENVO_00000305"/>
        <obo:RO_0001025 rdf:resource="http://purl.obolibrary.org/obo/GAZ_00045077"/>
        <obo:IAO_0000115>A cape marking the N tip of James Ross Island, which lies S of Trinity Peninsula.</obo:IAO_0000115>
        <oboInOwl:hasOBONamespace>GAZ</oboInOwl:hasOBONamespace>
        <oboInOwl:id>GAZ:00141538</oboInOwl:id>
        <rdfs:label>Cape Lachman</rdfs:label>
    </owl:NamedIndividual>
    


    <!-- http://purl.obolibrary.org/obo/GAZ_00141539 -->

    <owl:NamedIndividual rdf:about="http://purl.obolibrary.org/obo/GAZ_00141539">
        <rdf:type rdf:resource="http://purl.obolibrary.org/obo/ENVO_00000305"/>
        <obo:RO_0001025 rdf:resource="http://purl.obolibrary.org/obo/GAZ_00045077"/>
        <obo:IAO_0000115>A cape at the N side of the entrance to Rohss Bay, on the W side of James Ross Island.</obo:IAO_0000115>
        <oboInOwl:hasOBONamespace>GAZ</oboInOwl:hasOBONamespace>
        <oboInOwl:id>GAZ:00141539</oboInOwl:id>
        <rdfs:label>Cape Obelisk</rdfs:label>
    </owl:NamedIndividual>
    


    <!-- http://purl.obolibrary.org/obo/GAZ_00141552 -->

    <owl:NamedIndividual rdf:about="http://purl.obolibrary.org/obo/GAZ_00141552">
        <obo:RO_0001025 rdf:resource="http://purl.obolibrary.org/obo/GAZ_00000373"/>
        <obo:IAO_0000115>That area of the Southern Ocean from the N limit of the Bellingshausen Sea at 70WdegW to the W limit of the Weddell Sea at 65degW.</obo:IAO_0000115>
        <oboInOwl:hasOBONamespace>GAZ</oboInOwl:hasOBONamespace>
        <oboInOwl:id>GAZ:00141552</oboInOwl:id>
        <rdfs:label>Southern Ocean coastal western waters of Graham Land</rdfs:label>
    </owl:NamedIndividual>
    


    <!-- http://purl.obolibrary.org/obo/GAZ_00141553 -->

    <owl:NamedIndividual rdf:about="http://purl.obolibrary.org/obo/GAZ_00141553">
        <obo:RO_0001025 rdf:resource="http://purl.obolibrary.org/obo/GAZ_00141082"/>
        <obo:IAO_0000115>A small group of islands within Darbel Bay, lying just south of Darbel Islands off the west coast of Graham Land.</obo:IAO_0000115>
        <oboInOwl:hasOBONamespace>GAZ</oboInOwl:hasOBONamespace>
        <oboInOwl:id>GAZ:00141553</oboInOwl:id>
        <rdfs:label>Kidd Islands</rdfs:label>
    </owl:NamedIndividual>
    


    <!-- http://purl.obolibrary.org/obo/GAZ_00141554 -->

    <owl:NamedIndividual rdf:about="http://purl.obolibrary.org/obo/GAZ_00141554">
        <obo:RO_0001025 rdf:resource="http://purl.obolibrary.org/obo/GAZ_00000373"/>
        <obo:IAO_0000115>That part of the Southern Ocean, E of Cape Norvgica at 12degW and W 20degE.</obo:IAO_0000115>
        <oboInOwl:hasOBONamespace>GAZ</oboInOwl:hasOBONamespace>
        <oboInOwl:id>GAZ:00141554</oboInOwl:id>
        <rdfs:label>Southern Ocean coastal waters of western Dronning Maud Land</rdfs:label>
    </owl:NamedIndividual>
    


    <!-- http://purl.obolibrary.org/obo/GAZ_00141555 -->

    <owl:NamedIndividual rdf:about="http://purl.obolibrary.org/obo/GAZ_00141555">
        <obo:RO_0001025 rdf:resource="http://purl.obolibrary.org/obo/GAZ_00000373"/>
        <obo:IAO_0000115>That part of the Southern Ocean between the E limit of the Cosmonaut Sea, at 46degE, and the W limit of the Cooperation Sea, at approximately 57degE.</obo:IAO_0000115>
        <oboInOwl:hasOBONamespace>GAZ</oboInOwl:hasOBONamespace>
        <oboInOwl:id>GAZ:00141555</oboInOwl:id>
        <rdfs:label>Southern Ocean coastal waters of Enderby Land</rdfs:label>
    </owl:NamedIndividual>
    


    <!-- http://purl.obolibrary.org/obo/GAZ_00141556 -->

    <owl:NamedIndividual rdf:about="http://purl.obolibrary.org/obo/GAZ_00141556">
        <obo:RO_0001025 rdf:resource="http://purl.obolibrary.org/obo/GAZ_00000373"/>
        <obo:IAO_0000115>That part of the Southern Ocean between the E limit of the Amundsen Sea at approximately 126degW and the E limit of the Ross Sea at approximately 158degW, between Cape Dart on Sipple Island and Cape Colbeck.</obo:IAO_0000115>
        <oboInOwl:hasOBONamespace>GAZ</oboInOwl:hasOBONamespace>
        <oboInOwl:id>GAZ:00141556</oboInOwl:id>
        <rdfs:label>Southern Ocean coastal waters of Ruppert Coast</rdfs:label>
    </owl:NamedIndividual>
    


    <!-- http://purl.obolibrary.org/obo/GAZ_00141557 -->

    <owl:NamedIndividual rdf:about="http://purl.obolibrary.org/obo/GAZ_00141557">
        <obo:RO_0001025 rdf:resource="http://purl.obolibrary.org/obo/GAZ_00140159"/>
        <obo:IAO_0000115>An ice-covered island 15 miles long, lying in the Nickerson Ice Shelf on the coast of Marie Byrd Land.</obo:IAO_0000115>
        <oboInOwl:hasOBONamespace>GAZ</oboInOwl:hasOBONamespace>
        <oboInOwl:id>GAZ:00141557</oboInOwl:id>
        <rdfs:label>Newman Island</rdfs:label>
    </owl:NamedIndividual>
    


    <!-- http://purl.obolibrary.org/obo/GAZ_00141558 -->

    <owl:NamedIndividual rdf:about="http://purl.obolibrary.org/obo/GAZ_00141558">
        <obo:RO_0001025 rdf:resource="http://purl.obolibrary.org/obo/GAZ_00051498"/>
        <obo:IAO_0000115>That part of the Southern Ocean bounded by Sedovodden at about 20degE and Riiser-Larsen Halvoya at about 34degE.</obo:IAO_0000115>
        <oboInOwl:hasOBONamespace>GAZ</oboInOwl:hasOBONamespace>
        <oboInOwl:id>GAZ:00141558</oboInOwl:id>
        <rdfs:label>Riiser-Larsen Sea</rdfs:label>
    </owl:NamedIndividual>
    


    <!-- http://purl.obolibrary.org/obo/GAZ_00141559 -->

    <owl:NamedIndividual rdf:about="http://purl.obolibrary.org/obo/GAZ_00141559">
        <obo:RO_0001025 rdf:resource="http://purl.obolibrary.org/obo/GAZ_00141336"/>
        <obo:IAO_0000115>An iceport about 10 mi long and wide, marking a more-or-less permanent indentation in the front of the Ekstrom Ice Shelf on the coast of Queen Maud Land.</obo:IAO_0000115>
        <oboInOwl:hasOBONamespace>GAZ</oboInOwl:hasOBONamespace>
        <oboInOwl:id>GAZ:00141559</oboInOwl:id>
        <rdfs:label>Atka Iceport</rdfs:label>
    </owl:NamedIndividual>
    


    <!-- http://purl.obolibrary.org/obo/GAZ_00141560 -->

    <owl:NamedIndividual rdf:about="http://purl.obolibrary.org/obo/GAZ_00141560">
        <obo:RO_0001025 rdf:resource="http://purl.obolibrary.org/obo/GAZ_00051129"/>
        <obo:IAO_0000115>An ice-covered island in the West Ice Shelf. It rises to 200 m and is located 12 mi E of Mikhaylov Island.</obo:IAO_0000115>
        <oboInOwl:hasOBONamespace>GAZ</oboInOwl:hasOBONamespace>
        <oboInOwl:id>GAZ:00141560</oboInOwl:id>
        <rdfs:label>Zavadovskiy Island</rdfs:label>
    </owl:NamedIndividual>
    


    <!-- http://purl.obolibrary.org/obo/GAZ_00141561 -->

    <owl:NamedIndividual rdf:about="http://purl.obolibrary.org/obo/GAZ_00141561">
        <obo:RO_0001025 rdf:resource="http://purl.obolibrary.org/obo/GAZ_00003703"/>
        <obo:IAO_0000115>A high ice-covered island on the W side of the Amery Ice Shelf about 14 mi S of Landon Promontory.</obo:IAO_0000115>
        <oboInOwl:hasOBONamespace>GAZ</oboInOwl:hasOBONamespace>
        <oboInOwl:id>GAZ:00141561</oboInOwl:id>
        <rdfs:label>Single Island</rdfs:label>
    </owl:NamedIndividual>
    


    <!-- http://purl.obolibrary.org/obo/GAZ_00141562 -->

    <owl:NamedIndividual rdf:about="http://purl.obolibrary.org/obo/GAZ_00141562">
        <obo:RO_0001025 rdf:resource="http://purl.obolibrary.org/obo/GAZ_00141558"/>
        <obo:IAO_0000115>An iceport about 5 mi wide, which marks a more-or-less permanent indentation in the seaward front of the extensive ice shelf fringing the coast of Queen Maud Land.</obo:IAO_0000115>
        <oboInOwl:hasOBONamespace>GAZ</oboInOwl:hasOBONamespace>
        <oboInOwl:id>GAZ:00141562</oboInOwl:id>
        <rdfs:label>Godel Iceport</rdfs:label>
    </owl:NamedIndividual>
    


    <!-- http://purl.obolibrary.org/obo/GAZ_00141563 -->

    <owl:NamedIndividual rdf:about="http://purl.obolibrary.org/obo/GAZ_00141563">
        <obo:RO_0001025 rdf:resource="http://purl.obolibrary.org/obo/GAZ_00051499"/>
        <obo:IAO_0000115>A small bay at the eastern end of Sabrina Coast. The Henry Islands lie in the western part of the bay.</obo:IAO_0000115>
        <oboInOwl:hasOBONamespace>GAZ</oboInOwl:hasOBONamespace>
        <oboInOwl:id>GAZ:00141563</oboInOwl:id>
        <rdfs:label>Henry Bay</rdfs:label>
    </owl:NamedIndividual>
    


    <!-- http://purl.obolibrary.org/obo/GAZ_00141564 -->

    <owl:NamedIndividual rdf:about="http://purl.obolibrary.org/obo/GAZ_00141564">
        <obo:RO_0001025 rdf:resource="http://purl.obolibrary.org/obo/GAZ_00141563"/>
        <obo:IAO_0000115>A group of four small islands in the western part of Henry Bay.</obo:IAO_0000115>
        <oboInOwl:hasOBONamespace>GAZ</oboInOwl:hasOBONamespace>
        <oboInOwl:id>GAZ:00141564</oboInOwl:id>
        <rdfs:label>Henry Islands</rdfs:label>
    </owl:NamedIndividual>
    


    <!-- http://purl.obolibrary.org/obo/GAZ_00141565 -->

    <owl:NamedIndividual rdf:about="http://purl.obolibrary.org/obo/GAZ_00141565">
        <obo:RO_0001025 rdf:resource="http://purl.obolibrary.org/obo/GAZ_00045057"/>
        <obo:IAO_0000115>A small ice-covered island, lying at the seaward extremity of Shackleton Ice Shelf, between the projections of Denman and Scott Glaciers.</obo:IAO_0000115>
        <oboInOwl:hasOBONamespace>GAZ</oboInOwl:hasOBONamespace>
        <oboInOwl:id>GAZ:00141565</oboInOwl:id>
        <rdfs:label>Chugunov Island</rdfs:label>
    </owl:NamedIndividual>
    


    <!-- http://purl.obolibrary.org/obo/GAZ_00141566 -->

    <owl:NamedIndividual rdf:about="http://purl.obolibrary.org/obo/GAZ_00141566">
        <obo:RO_0001025 rdf:resource="http://purl.obolibrary.org/obo/GAZ_00051499"/>
        <obo:IAO_0000115>An ice-filled bay indenting the coast just east of Cape Lewis.</obo:IAO_0000115>
        <oboInOwl:hasOBONamespace>GAZ</oboInOwl:hasOBONamespace>
        <oboInOwl:id>GAZ:00141566</oboInOwl:id>
        <rdfs:label>Maury Bay</rdfs:label>
    </owl:NamedIndividual>
    


    <!-- http://purl.obolibrary.org/obo/GAZ_00141567 -->

    <owl:NamedIndividual rdf:about="http://purl.obolibrary.org/obo/GAZ_00141567">
        <rdf:type rdf:resource="http://purl.obolibrary.org/obo/ENVO_00000032"/>
        <obo:RO_0001025 rdf:resource="http://purl.obolibrary.org/obo/GAZ_00051499"/>
        <obo:IAO_0000115>An embayment about 14 mi wide between the eastern side of the Mertz Glacier Tongue and the mainland.</obo:IAO_0000115>
        <oboInOwl:hasOBONamespace>GAZ</oboInOwl:hasOBONamespace>
        <oboInOwl:id>GAZ:00141567</oboInOwl:id>
        <rdfs:label>Fisher Bay</rdfs:label>
    </owl:NamedIndividual>
    


    <!-- http://purl.obolibrary.org/obo/GAZ_00141568 -->

    <owl:NamedIndividual rdf:about="http://purl.obolibrary.org/obo/GAZ_00141568">
        <obo:RO_0001025 rdf:resource="http://purl.obolibrary.org/obo/GAZ_00051499"/>
        <obo:IAO_0000115>An ice shelf along the coast of Antarctica between Mawson Peninsula and Cape Andreyev.</obo:IAO_0000115>
        <oboInOwl:hasOBONamespace>GAZ</oboInOwl:hasOBONamespace>
        <oboInOwl:id>GAZ:00141568</oboInOwl:id>
        <rdfs:label>Slava Ice Shelf</rdfs:label>
    </owl:NamedIndividual>
    


    <!-- http://purl.obolibrary.org/obo/GAZ_00141569 -->

    <owl:NamedIndividual rdf:about="http://purl.obolibrary.org/obo/GAZ_00141569">
        <obo:RO_0001025 rdf:resource="http://purl.obolibrary.org/obo/GAZ_00051499"/>
        <obo:IAO_0000115>A bay on the coast, 10 mi wide, between Drake Head and Cape Kinsey.</obo:IAO_0000115>
        <oboInOwl:hasOBONamespace>GAZ</oboInOwl:hasOBONamespace>
        <oboInOwl:id>GAZ:00141569</oboInOwl:id>
        <rdfs:label>Davies Bay</rdfs:label>
    </owl:NamedIndividual>
    


    <!-- http://purl.obolibrary.org/obo/GAZ_00141570 -->

    <owl:NamedIndividual rdf:about="http://purl.obolibrary.org/obo/GAZ_00141570">
        <obo:RO_0001025 rdf:resource="http://purl.obolibrary.org/obo/GAZ_00023304"/>
        <obo:IAO_0000115>A bay just N of Cape Chocolate along the coast of Victoria Land.</obo:IAO_0000115>
        <oboInOwl:hasOBONamespace>GAZ</oboInOwl:hasOBONamespace>
        <oboInOwl:id>GAZ:00141570</oboInOwl:id>
        <rdfs:label>Salmon Bay</rdfs:label>
    </owl:NamedIndividual>
    


    <!-- http://purl.obolibrary.org/obo/GAZ_00141571 -->

    <owl:NamedIndividual rdf:about="http://purl.obolibrary.org/obo/GAZ_00141571">
        <obo:RO_0001025 rdf:resource="http://purl.obolibrary.org/obo/GAZ_00023304"/>
        <obo:IAO_0000115>A reentrant about 17 mi wide occupied by the lower part of Byrd Glacier, lying between Cape Kerr and Cape Selborne on the W side of the Ross Ice Shelf.</obo:IAO_0000115>
        <oboInOwl:hasOBONamespace>GAZ</oboInOwl:hasOBONamespace>
        <oboInOwl:id>GAZ:00141571</oboInOwl:id>
        <rdfs:label>Barne Inlet</rdfs:label>
    </owl:NamedIndividual>
    


    <!-- http://purl.obolibrary.org/obo/GAZ_00141572 -->

    <owl:NamedIndividual rdf:about="http://purl.obolibrary.org/obo/GAZ_00141572">
        <rdf:type rdf:resource="http://purl.obolibrary.org/obo/ENVO_00000032"/>
        <obo:RO_0001025 rdf:resource="http://purl.obolibrary.org/obo/GAZ_00141556"/>
        <obo:IAO_0000115>An embayment about 115 mi wide along the coastline of Antarctica, lying seaward of the Getz Ice Shelf. Nearly a right angle in plan, its limits are described by Grant, Dean, and Siple Islands, which are partially or wholly embedded in the ice shelf.</obo:IAO_0000115>
        <oboInOwl:hasOBONamespace>GAZ</oboInOwl:hasOBONamespace>
        <oboInOwl:id>GAZ:00141572</oboInOwl:id>
        <rdfs:label>Wrigley Gulf</rdfs:label>
    </owl:NamedIndividual>
    


    <!-- http://purl.obolibrary.org/obo/GAZ_00141573 -->

    <owl:NamedIndividual rdf:about="http://purl.obolibrary.org/obo/GAZ_00141573">
        <obo:RO_0001025 rdf:resource="http://purl.obolibrary.org/obo/GAZ_00014085"/>
        <obo:IAO_0000115>A very large and rather compact iceberg tongue which is aground and lies in the Amundsen Sea, about 20 mi NE of Bear Peninsula, Marie Byrd Land. The feature is about 70 mi long and 20 mi wide and in 1966-01 its S end was only 3 mi N of Thwaites Glacier Tongue, from whence it had broken off.</obo:IAO_0000115>
        <oboInOwl:hasOBONamespace>GAZ</oboInOwl:hasOBONamespace>
        <oboInOwl:id>GAZ:00141573</oboInOwl:id>
        <rdfs:label>Thwaites Iceberg Tongue</rdfs:label>
    </owl:NamedIndividual>
    


    <!-- http://purl.obolibrary.org/obo/GAZ_00141574 -->

    <owl:NamedIndividual rdf:about="http://purl.obolibrary.org/obo/GAZ_00141574">
        <obo:RO_0001025 rdf:resource="http://purl.obolibrary.org/obo/GAZ_00140310"/>
        <obo:IAO_0000115>An island 0.8 km across, lying 2.4 km east of Lang Island, close east of the Oygarden Group and Edward VIII Bay.</obo:IAO_0000115>
        <oboInOwl:hasOBONamespace>GAZ</oboInOwl:hasOBONamespace>
        <oboInOwl:id>GAZ:00141574</oboInOwl:id>
        <rdfs:label>Abrupt Island</rdfs:label>
    </owl:NamedIndividual>
    


    <!-- http://purl.obolibrary.org/obo/GAZ_00141575 -->

    <owl:NamedIndividual rdf:about="http://purl.obolibrary.org/obo/GAZ_00141575">
        <obo:RO_0001025 rdf:resource="http://purl.obolibrary.org/obo/GAZ_00140310"/>
        <obo:IAO_0000115>An island 1.6 km long and 0.6 km wide, lying midway between Abrupt Island and the Oygarden Group.</obo:IAO_0000115>
        <oboInOwl:hasOBONamespace>GAZ</oboInOwl:hasOBONamespace>
        <oboInOwl:id>GAZ:00141575</oboInOwl:id>
        <rdfs:label>Lang Island</rdfs:label>
    </owl:NamedIndividual>
    


    <!-- http://purl.obolibrary.org/obo/GAZ_00141576 -->

    <owl:NamedIndividual rdf:about="http://purl.obolibrary.org/obo/GAZ_00141576">
        <obo:RO_0001025 rdf:resource="http://purl.obolibrary.org/obo/GAZ_00140885"/>
        <obo:IAO_0000115>An island 2.4 km long, lying 1.6 km west of Shaula Island in the Oygarden Group.</obo:IAO_0000115>
        <oboInOwl:hasOBONamespace>GAZ</oboInOwl:hasOBONamespace>
        <oboInOwl:id>GAZ:00141576</oboInOwl:id>
        <rdfs:label>Achernar Island</rdfs:label>
    </owl:NamedIndividual>
    


    <!-- http://purl.obolibrary.org/obo/GAZ_00141577 -->

    <owl:NamedIndividual rdf:about="http://purl.obolibrary.org/obo/GAZ_00141577">
        <obo:RO_0001025 rdf:resource="http://purl.obolibrary.org/obo/GAZ_00140885"/>
        <obo:IAO_0000115>An island 4.8 km long and rising to 150 m, lying 1.6 km east of Achernar Island in the Oygarden Group.</obo:IAO_0000115>
        <oboInOwl:hasOBONamespace>GAZ</oboInOwl:hasOBONamespace>
        <oboInOwl:id>GAZ:00141577</oboInOwl:id>
        <rdfs:label>Shaula Island</rdfs:label>
    </owl:NamedIndividual>
    


    <!-- http://purl.obolibrary.org/obo/GAZ_00141578 -->

    <owl:NamedIndividual rdf:about="http://purl.obolibrary.org/obo/GAZ_00141578">
        <obo:RO_0001025 rdf:resource="http://purl.obolibrary.org/obo/GAZ_00014089"/>
        <obo:IAO_0000115>A small group of islands lying 8 mi N of Cape Berteaux, off the W coast of Graham Land.</obo:IAO_0000115>
        <oboInOwl:hasOBONamespace>GAZ</oboInOwl:hasOBONamespace>
        <oboInOwl:id>GAZ:00141578</oboInOwl:id>
        <rdfs:label>Terra Firma Islands</rdfs:label>
    </owl:NamedIndividual>
    


    <!-- http://purl.obolibrary.org/obo/GAZ_00141579 -->

    <owl:NamedIndividual rdf:about="http://purl.obolibrary.org/obo/GAZ_00141579">
        <obo:RO_0001025 rdf:resource="http://purl.obolibrary.org/obo/GAZ_00141578"/>
        <obo:IAO_0000115>The largest and southeasternmost of the Terra Firma Islands, with steep rocky cliffs surmounted by a rock and snow cone rising to 320 m, lying in Marguerite Bay off the west coast of Graham Land.</obo:IAO_0000115>
        <oboInOwl:hasOBONamespace>GAZ</oboInOwl:hasOBONamespace>
        <oboInOwl:id>GAZ:00141579</oboInOwl:id>
        <rdfs:label>Alamode Island</rdfs:label>
    </owl:NamedIndividual>
    


    <!-- http://purl.obolibrary.org/obo/GAZ_00141580 -->

    <owl:NamedIndividual rdf:about="http://purl.obolibrary.org/obo/GAZ_00141580">
        <obo:RO_0001025 rdf:resource="http://purl.obolibrary.org/obo/GAZ_00141552"/>
        <obo:IAO_0000115>A small group of ice-covered islands lying close off the front of Wordie Ice Shelf and between 4 and 11 mi NW of Mount Guernsey, off the W coast of Antarctic Peninsula.</obo:IAO_0000115>
        <oboInOwl:hasOBONamespace>GAZ</oboInOwl:hasOBONamespace>
        <oboInOwl:id>GAZ:00141580</oboInOwl:id>
        <rdfs:label>Bugge Islands</rdfs:label>
    </owl:NamedIndividual>
    


    <!-- http://purl.obolibrary.org/obo/GAZ_00141581 -->

    <owl:NamedIndividual rdf:about="http://purl.obolibrary.org/obo/GAZ_00141581">
        <obo:RO_0001025 rdf:resource="http://purl.obolibrary.org/obo/GAZ_00141580"/>
        <obo:IAO_0000115>The central of the three Bugge Islands, off Wordie Ice Shelf, Fallieres Coast, Antarctic Peninsula.</obo:IAO_0000115>
        <oboInOwl:hasOBONamespace>GAZ</oboInOwl:hasOBONamespace>
        <oboInOwl:id>GAZ:00141581</oboInOwl:id>
        <rdfs:label>Aldea Island</rdfs:label>
    </owl:NamedIndividual>
    


    <!-- http://purl.obolibrary.org/obo/GAZ_00141582 -->

    <owl:NamedIndividual rdf:about="http://purl.obolibrary.org/obo/GAZ_00141582">
        <obo:RO_0001025 rdf:resource="http://purl.obolibrary.org/obo/GAZ_00045121"/>
        <obo:IAO_0000115>The westernmost point of Adery island.</obo:IAO_0000115>
        <oboInOwl:hasOBONamespace>GAZ</oboInOwl:hasOBONamespace>
        <oboInOwl:id>GAZ:00141582</oboInOwl:id>
        <rdfs:label>Mast Point</rdfs:label>
    </owl:NamedIndividual>
    


    <!-- http://purl.obolibrary.org/obo/GAZ_00141583 -->

    <owl:NamedIndividual rdf:about="http://purl.obolibrary.org/obo/GAZ_00141583">
        <obo:RO_0001025 rdf:resource="http://purl.obolibrary.org/obo/GAZ_00014108"/>
        <obo:IAO_0000115>The water passage between Ardery Island and Holl and Ford Islands to the south.</obo:IAO_0000115>
        <oboInOwl:hasOBONamespace>GAZ</oboInOwl:hasOBONamespace>
        <oboInOwl:id>GAZ:00141583</oboInOwl:id>
        <rdfs:label>Hiegel Passage</rdfs:label>
    </owl:NamedIndividual>
    


    <!-- http://purl.obolibrary.org/obo/GAZ_00141584 -->

    <owl:NamedIndividual rdf:about="http://purl.obolibrary.org/obo/GAZ_00141584">
        <rdf:type rdf:resource="http://purl.obolibrary.org/obo/ENVO_00000029"/>
        <obo:RO_0001025 rdf:resource="http://purl.obolibrary.org/obo/GAZ_00045121"/>
        <obo:IAO_0000115>A ravine in the western part of Ardery Island.</obo:IAO_0000115>
        <oboInOwl:hasOBONamespace>GAZ</oboInOwl:hasOBONamespace>
        <oboInOwl:id>GAZ:00141584</oboInOwl:id>
        <rdfs:label>Cave Ravine</rdfs:label>
    </owl:NamedIndividual>
    


    <!-- http://purl.obolibrary.org/obo/GAZ_00141585 -->

    <owl:NamedIndividual rdf:about="http://purl.obolibrary.org/obo/GAZ_00141585">
        <obo:RO_0001025 rdf:resource="http://purl.obolibrary.org/obo/GAZ_00045050"/>
        <obo:IAO_0000115>The southernmost island in the Debenham Islands, off the west coast of Graham Land.</obo:IAO_0000115>
        <oboInOwl:hasOBONamespace>GAZ</oboInOwl:hasOBONamespace>
        <oboInOwl:id>GAZ:00141585</oboInOwl:id>
        <rdfs:label>Audrey Island</rdfs:label>
    </owl:NamedIndividual>
    


    <!-- http://purl.obolibrary.org/obo/GAZ_00141586 -->

    <owl:NamedIndividual rdf:about="http://purl.obolibrary.org/obo/GAZ_00141586">
        <obo:RO_0001025 rdf:resource="http://purl.obolibrary.org/obo/GAZ_00139422"/>
        <obo:IAO_0000115>A group of small islands extending 16 km in an east-west direction, lying close northwest of Cape Daly.</obo:IAO_0000115>
        <oboInOwl:hasOBONamespace>GAZ</oboInOwl:hasOBONamespace>
        <oboInOwl:id>GAZ:00141586</oboInOwl:id>
        <rdfs:label>Robinson Group</rdfs:label>
    </owl:NamedIndividual>
    


    <!-- http://purl.obolibrary.org/obo/GAZ_00141587 -->

    <owl:NamedIndividual rdf:about="http://purl.obolibrary.org/obo/GAZ_00141587">
        <obo:RO_0001025 rdf:resource="http://purl.obolibrary.org/obo/GAZ_00141586"/>
        <obo:IAO_0000115>A group of small islands at northeast end of the Robinson Group, located 9 km north of Cape Daly, Mac Robertson Land.</obo:IAO_0000115>
        <oboInOwl:hasOBONamespace>GAZ</oboInOwl:hasOBONamespace>
        <oboInOwl:id>GAZ:00141587</oboInOwl:id>
        <rdfs:label>Auster Islands</rdfs:label>
    </owl:NamedIndividual>
    


    <!-- http://purl.obolibrary.org/obo/GAZ_00141588 -->

    <owl:NamedIndividual rdf:about="http://purl.obolibrary.org/obo/GAZ_00141588">
        <obo:RO_0001025 rdf:resource="http://purl.obolibrary.org/obo/GAZ_00051499"/>
        <obo:IAO_0000115>A group of small rocky islands lying 4.8 km north of Cape Kinsey and the Wilson Hills.</obo:IAO_0000115>
        <oboInOwl:hasOBONamespace>GAZ</oboInOwl:hasOBONamespace>
        <oboInOwl:id>GAZ:00141588</oboInOwl:id>
        <rdfs:label>Aviation Islands</rdfs:label>
    </owl:NamedIndividual>
    


    <!-- http://purl.obolibrary.org/obo/GAZ_00141589 -->

    <owl:NamedIndividual rdf:about="http://purl.obolibrary.org/obo/GAZ_00141589">
        <obo:RO_0001025 rdf:resource="http://purl.obolibrary.org/obo/GAZ_00045065"/>
        <obo:IAO_0000115>A group of 4 small islands lying 1.6 km northwest of Parallactic Islands in Holme Bay, Mac Robertson Land; they share their name with the largest island in the group.</obo:IAO_0000115>
        <oboInOwl:hasOBONamespace>GAZ</oboInOwl:hasOBONamespace>
        <oboInOwl:id>GAZ:00141589</oboInOwl:id>
        <rdfs:label>Azimuth Islands</rdfs:label>
    </owl:NamedIndividual>
    


    <!-- http://purl.obolibrary.org/obo/GAZ_00141590 -->

    <owl:NamedIndividual rdf:about="http://purl.obolibrary.org/obo/GAZ_00141590">
        <obo:RO_0001025 rdf:resource="http://purl.obolibrary.org/obo/GAZ_00141589"/>
        <obo:IAO_0000115>The largest of the Azimuth Islands lying in Holme Bay, Mac Robertson Land.</obo:IAO_0000115>
        <oboInOwl:hasOBONamespace>GAZ</oboInOwl:hasOBONamespace>
        <oboInOwl:id>GAZ:00141590</oboInOwl:id>
        <rdfs:label>Azimuth Island</rdfs:label>
    </owl:NamedIndividual>
    


    <!-- http://purl.obolibrary.org/obo/GAZ_00141591 -->

    <owl:NamedIndividual rdf:about="http://purl.obolibrary.org/obo/GAZ_00141591">
        <obo:RO_0001025 rdf:resource="http://purl.obolibrary.org/obo/GAZ_00045065"/>
        <obo:IAO_0000115>Two small islands 0.5 mi S of the Parallactic Islands in Holme Bay, Mac Robertson Land.</obo:IAO_0000115>
        <oboInOwl:hasOBONamespace>GAZ</oboInOwl:hasOBONamespace>
        <oboInOwl:id>GAZ:00141591</oboInOwl:id>
        <rdfs:label>Kellas Islands</rdfs:label>
    </owl:NamedIndividual>
    


    <!-- http://purl.obolibrary.org/obo/GAZ_00141592 -->

    <owl:NamedIndividual rdf:about="http://purl.obolibrary.org/obo/GAZ_00141592">
        <obo:RO_0001025 rdf:resource="http://purl.obolibrary.org/obo/GAZ_00045065"/>
        <obo:IAO_0000115>A group of 6 small islands between the Azimuth and Kellas Islands in Holme Bay, Mac Robertson Land.</obo:IAO_0000115>
        <oboInOwl:hasOBONamespace>GAZ</oboInOwl:hasOBONamespace>
        <oboInOwl:id>GAZ:00141592</oboInOwl:id>
        <rdfs:label>Parallactic Islands</rdfs:label>
    </owl:NamedIndividual>
    


    <!-- http://purl.obolibrary.org/obo/GAZ_00141593 -->

    <owl:NamedIndividual rdf:about="http://purl.obolibrary.org/obo/GAZ_00141593">
        <obo:RO_0001025 rdf:resource="http://purl.obolibrary.org/obo/GAZ_00023294"/>
        <obo:IAO_0000115>A small island 1.6 km west of Rundvags Head in the southeast part of Lutzow-Holm Bay.</obo:IAO_0000115>
        <oboInOwl:hasOBONamespace>GAZ</oboInOwl:hasOBONamespace>
        <oboInOwl:id>GAZ:00141593</oboInOwl:id>
        <rdfs:label>Azuki Island</rdfs:label>
    </owl:NamedIndividual>
    


    <!-- http://purl.obolibrary.org/obo/GAZ_00141594 -->

    <owl:NamedIndividual rdf:about="http://purl.obolibrary.org/obo/GAZ_00141594">
        <obo:RO_0001025 rdf:resource="http://purl.obolibrary.org/obo/GAZ_00014108"/>
        <obo:IAO_0000115>A sheltered bay about 1 mi in extent, between Clark Peninsula and Bailey Peninsula in the Windmill Islands.</obo:IAO_0000115>
        <oboInOwl:hasOBONamespace>GAZ</oboInOwl:hasOBONamespace>
        <oboInOwl:id>GAZ:00141594</oboInOwl:id>
        <rdfs:label>Newcomb Bay</rdfs:label>
    </owl:NamedIndividual>
    


    <!-- http://purl.obolibrary.org/obo/GAZ_00141595 -->

    <owl:NamedIndividual rdf:about="http://purl.obolibrary.org/obo/GAZ_00141595">
        <obo:RO_0001025 rdf:resource="http://purl.obolibrary.org/obo/GAZ_00045034"/>
        <obo:IAO_0000115>An island in Antarctica, 3.2 km long and 1.6 km wide, situated on the south flank of Beaver Glacier in Amundsen Bay.</obo:IAO_0000115>
        <oboInOwl:hasOBONamespace>GAZ</oboInOwl:hasOBONamespace>
        <oboInOwl:id>GAZ:00141595</oboInOwl:id>
        <rdfs:label>Beaver Island</rdfs:label>
    </owl:NamedIndividual>
    


    <!-- http://purl.obolibrary.org/obo/GAZ_00141596 -->

    <owl:NamedIndividual rdf:about="http://purl.obolibrary.org/obo/GAZ_00141596">
        <obo:RO_0001025 rdf:resource="http://purl.obolibrary.org/obo/GAZ_00051128"/>
        <obo:IAO_0000115>A group of islands at the southwest side of Liard Island in Hanusse Bay, extending in a southwest direction for 10 km off the west coast of Graham Land.</obo:IAO_0000115>
        <oboInOwl:hasOBONamespace>GAZ</oboInOwl:hasOBONamespace>
        <oboInOwl:id>GAZ:00141596</oboInOwl:id>
        <rdfs:label>Bennett Islands</rdfs:label>
    </owl:NamedIndividual>
    


    <!-- http://purl.obolibrary.org/obo/GAZ_00141597 -->

    <owl:NamedIndividual rdf:about="http://purl.obolibrary.org/obo/GAZ_00141597">
        <obo:RO_0001025 rdf:resource="http://purl.obolibrary.org/obo/GAZ_00014108"/>
        <obo:IAO_0000115>A body of water separating Mitchell Peninsula from Pidgeon Island and Warrington Island.</obo:IAO_0000115>
        <oboInOwl:hasOBONamespace>GAZ</oboInOwl:hasOBONamespace>
        <oboInOwl:id>GAZ:00141597</oboInOwl:id>
        <rdfs:label>Robertson Channel</rdfs:label>
    </owl:NamedIndividual>
    


    <!-- http://purl.obolibrary.org/obo/GAZ_00141598 -->

    <owl:NamedIndividual rdf:about="http://purl.obolibrary.org/obo/GAZ_00141598">
        <obo:RO_0001025 rdf:resource="http://purl.obolibrary.org/obo/GAZ_00014094"/>
        <obo:IAO_0000115>A rocky island, 0.7 mi long, lying immediately S of Pidgeon Island in the Windmill Islands.</obo:IAO_0000115>
        <oboInOwl:hasOBONamespace>GAZ</oboInOwl:hasOBONamespace>
        <oboInOwl:id>GAZ:00141598</oboInOwl:id>
        <rdfs:label>Warrington Island</rdfs:label>
    </owl:NamedIndividual>
    


    <!-- http://purl.obolibrary.org/obo/GAZ_00141599 -->

    <owl:NamedIndividual rdf:about="http://purl.obolibrary.org/obo/GAZ_00141599">
        <obo:RO_0001025 rdf:resource="http://purl.obolibrary.org/obo/GAZ_00014094"/>
        <obo:IAO_0000115>A rocky island, 0.8 mi long, lying immediately S of Hollin Island in the Windmill Islands.</obo:IAO_0000115>
        <oboInOwl:hasOBONamespace>GAZ</oboInOwl:hasOBONamespace>
        <oboInOwl:id>GAZ:00141599</oboInOwl:id>
        <rdfs:label>Midgley Island</rdfs:label>
    </owl:NamedIndividual>
    


    <!-- http://purl.obolibrary.org/obo/GAZ_00141600 -->

    <owl:NamedIndividual rdf:about="http://purl.obolibrary.org/obo/GAZ_00141600">
        <obo:RO_0001025 rdf:resource="http://purl.obolibrary.org/obo/GAZ_00014094"/>
        <obo:IAO_0000115>Several tidal and submerged rocks among the islands lying off the W side of Midgley Island, in the Windmill Islands.</obo:IAO_0000115>
        <oboInOwl:hasOBONamespace>GAZ</oboInOwl:hasOBONamespace>
        <oboInOwl:id>GAZ:00141600</oboInOwl:id>
        <rdfs:label>Midgley Reefs</rdfs:label>
    </owl:NamedIndividual>
    


    <!-- http://purl.obolibrary.org/obo/GAZ_00141601 -->

    <owl:NamedIndividual rdf:about="http://purl.obolibrary.org/obo/GAZ_00141601">
        <obo:RO_0001025 rdf:resource="http://purl.obolibrary.org/obo/GAZ_00011769"/>
        <obo:IAO_0000115>A small island lying at the N tip of Brown Peninsula in the Ross Ice Shelf.</obo:IAO_0000115>
        <oboInOwl:hasOBONamespace>GAZ</oboInOwl:hasOBONamespace>
        <oboInOwl:id>GAZ:00141601</oboInOwl:id>
        <rdfs:label>Bratina Island</rdfs:label>
    </owl:NamedIndividual>
    


    <!-- http://purl.obolibrary.org/obo/GAZ_00141602 -->

    <owl:NamedIndividual rdf:about="http://purl.obolibrary.org/obo/GAZ_00141602">
        <obo:RO_0001025 rdf:resource="http://purl.obolibrary.org/obo/GAZ_00051527"/>
        <obo:IAO_0000115>An island, part of the Melchior Islands in the Southern Ocean along the west coast of the Antarctic Peninsula.</obo:IAO_0000115>
        <oboInOwl:hasOBONamespace>GAZ</oboInOwl:hasOBONamespace>
        <oboInOwl:id>GAZ:00141602</oboInOwl:id>
        <rdfs:label>Bremen Island</rdfs:label>
    </owl:NamedIndividual>
    


    <!-- http://purl.obolibrary.org/obo/GAZ_00141603 -->

    <owl:NamedIndividual rdf:about="http://purl.obolibrary.org/obo/GAZ_00141603">
        <obo:RO_0001025 rdf:resource="http://purl.obolibrary.org/obo/GAZ_00051528"/>
        <obo:IAO_0000115>A channel that separates Omega Island and Bremen Island.</obo:IAO_0000115>
        <oboInOwl:hasOBONamespace>GAZ</oboInOwl:hasOBONamespace>
        <oboInOwl:id>GAZ:00141603</oboInOwl:id>
        <rdfs:label>Bremenkanal</rdfs:label>
    </owl:NamedIndividual>
    


    <!-- http://purl.obolibrary.org/obo/GAZ_00141604 -->

    <owl:NamedIndividual rdf:about="http://purl.obolibrary.org/obo/GAZ_00141604">
        <obo:RO_0001025 rdf:resource="http://purl.obolibrary.org/obo/GAZ_00141556"/>
        <obo:IAO_0000115>A rocky, but mostly snow-covered island about 50 miles north-northeast of the mouth of Land Glacier off the coast of Marie Byrd Land.</obo:IAO_0000115>
        <oboInOwl:hasOBONamespace>GAZ</oboInOwl:hasOBONamespace>
        <oboInOwl:id>GAZ:00141604</oboInOwl:id>
        <rdfs:label>Cruzen Island</rdfs:label>
    </owl:NamedIndividual>
    


    <!-- http://purl.obolibrary.org/obo/GAZ_00141605 -->

    <owl:NamedIndividual rdf:about="http://purl.obolibrary.org/obo/GAZ_00141605">
        <obo:RO_0001025 rdf:resource="http://purl.obolibrary.org/obo/GAZ_00051525"/>
        <obo:IAO_0000115>The largest and westernmost of the Dailey Islands, located 5 miles northeast of Cape Chocolate.</obo:IAO_0000115>
        <oboInOwl:hasOBONamespace>GAZ</oboInOwl:hasOBONamespace>
        <oboInOwl:id>GAZ:00141605</oboInOwl:id>
        <rdfs:label>West Dailey Island</rdfs:label>
    </owl:NamedIndividual>
    


    <!-- http://purl.obolibrary.org/obo/GAZ_00141606 -->

    <owl:NamedIndividual rdf:about="http://purl.obolibrary.org/obo/GAZ_00141606">
        <obo:RO_0001025 rdf:resource="http://purl.obolibrary.org/obo/GAZ_00051525"/>
        <obo:IAO_0000115>An island 1.5 miles east of West Dailey Island.</obo:IAO_0000115>
        <oboInOwl:hasOBONamespace>GAZ</oboInOwl:hasOBONamespace>
        <oboInOwl:id>GAZ:00141606</oboInOwl:id>
        <rdfs:label>Juergens Island</rdfs:label>
    </owl:NamedIndividual>
    


    <!-- http://purl.obolibrary.org/obo/GAZ_00141607 -->

    <owl:NamedIndividual rdf:about="http://purl.obolibrary.org/obo/GAZ_00141607">
        <obo:RO_0001025 rdf:resource="http://purl.obolibrary.org/obo/GAZ_00051525"/>
        <obo:IAO_0000115>An island 0.5 miles long that is the easternmost feature in the Dailey Islands.</obo:IAO_0000115>
        <oboInOwl:hasOBONamespace>GAZ</oboInOwl:hasOBONamespace>
        <oboInOwl:id>GAZ:00141607</oboInOwl:id>
        <rdfs:label>Uberuaga Island</rdfs:label>
    </owl:NamedIndividual>
    


    <!-- http://purl.obolibrary.org/obo/GAZ_00141608 -->

    <owl:NamedIndividual rdf:about="http://purl.obolibrary.org/obo/GAZ_00141608">
        <obo:RO_0001025 rdf:resource="http://purl.obolibrary.org/obo/GAZ_00051525"/>
        <obo:IAO_0000115>An island n the east side of Juergens Island, 2 miles east of West Dailey Island.</obo:IAO_0000115>
        <oboInOwl:hasOBONamespace>GAZ</oboInOwl:hasOBONamespace>
        <oboInOwl:id>GAZ:00141608</oboInOwl:id>
        <rdfs:label>Hatcher Island</rdfs:label>
    </owl:NamedIndividual>
    


    <!-- http://purl.obolibrary.org/obo/GAZ_00141609 -->

    <owl:NamedIndividual rdf:about="http://purl.obolibrary.org/obo/GAZ_00141609">
        <obo:RO_0001025 rdf:resource="http://purl.obolibrary.org/obo/GAZ_00051525"/>
        <obo:IAO_0000115>An island lying 1 miles northwest of Uberuaga Island that is the northernmost feature in the Dailey Islands.</obo:IAO_0000115>
        <oboInOwl:hasOBONamespace>GAZ</oboInOwl:hasOBONamespace>
        <oboInOwl:id>GAZ:00141609</oboInOwl:id>
        <rdfs:label>Kuechle Island</rdfs:label>
    </owl:NamedIndividual>
    


    <!-- http://purl.obolibrary.org/obo/GAZ_00141610 -->

    <owl:NamedIndividual rdf:about="http://purl.obolibrary.org/obo/GAZ_00141610">
        <obo:RO_0001025 rdf:resource="http://purl.obolibrary.org/obo/GAZ_00140214"/>
        <obo:IAO_0000115>A narrow island which is the southernmost of the Sostrene Islands. The island is ice covered except for a small rock outcrop and barely protrudes above the general level of the Publications Ice Shelf.</obo:IAO_0000115>
        <oboInOwl:hasOBONamespace>GAZ</oboInOwl:hasOBONamespace>
        <oboInOwl:id>GAZ:00141610</oboInOwl:id>
        <rdfs:label>Debutante Island</rdfs:label>
    </owl:NamedIndividual>
    


    <!-- http://purl.obolibrary.org/obo/GAZ_00141611 -->

    <owl:NamedIndividual rdf:about="http://purl.obolibrary.org/obo/GAZ_00141611">
        <obo:RO_0001025 rdf:resource="http://purl.obolibrary.org/obo/GAZ_00141612"/>
        <obo:IAO_0000115>A narrow, ice-covered island 16 miles long, lying in Block Bay along the coast of Marie Byrd Land.</obo:IAO_0000115>
        <oboInOwl:hasOBONamespace>GAZ</oboInOwl:hasOBONamespace>
        <oboInOwl:id>GAZ:00141611</oboInOwl:id>
        <rdfs:label>Driscoll Island</rdfs:label>
    </owl:NamedIndividual>
    


    <!-- http://purl.obolibrary.org/obo/GAZ_00141612 -->

    <owl:NamedIndividual rdf:about="http://purl.obolibrary.org/obo/GAZ_00141612">
        <obo:RO_0001025 rdf:resource="http://purl.obolibrary.org/obo/GAZ_00141556"/>
        <obo:IAO_0000115>A long ice-filled bay lying E of Guest Peninsula along the coast of Marie Byrd Land.</obo:IAO_0000115>
        <oboInOwl:hasOBONamespace>GAZ</oboInOwl:hasOBONamespace>
        <oboInOwl:id>GAZ:00141612</oboInOwl:id>
        <rdfs:label>Block Bay</rdfs:label>
    </owl:NamedIndividual>
    


    <!-- http://purl.obolibrary.org/obo/GAZ_00141613 -->

    <owl:NamedIndividual rdf:about="http://purl.obolibrary.org/obo/GAZ_00141613">
        <obo:RO_0001025 rdf:resource="http://purl.obolibrary.org/obo/GAZ_00140365"/>
        <obo:IAO_0000115>A mountainous ice-free island, 2.5 miles long, lying in the southern part of Robertson Bay, along the northern coast of Victoria Land.</obo:IAO_0000115>
        <oboInOwl:hasOBONamespace>GAZ</oboInOwl:hasOBONamespace>
        <oboInOwl:id>GAZ:00141613</oboInOwl:id>
        <rdfs:label>Duke of York Island</rdfs:label>
    </owl:NamedIndividual>
    


    <!-- http://purl.obolibrary.org/obo/GAZ_00141614 -->

    <owl:NamedIndividual rdf:about="http://purl.obolibrary.org/obo/GAZ_00141614">
        <obo:RO_0001025 rdf:resource="http://purl.obolibrary.org/obo/GAZ_00051499"/>
        <obo:IAO_0000115>An anchorage lying immediately off Cape Margerie.</obo:IAO_0000115>
        <oboInOwl:hasOBONamespace>GAZ</oboInOwl:hasOBONamespace>
        <oboInOwl:id>GAZ:00141614</oboInOwl:id>
        <rdfs:label>Port Martin</rdfs:label>
    </owl:NamedIndividual>
    


    <!-- http://purl.obolibrary.org/obo/GAZ_00141615 -->

    <owl:NamedIndividual rdf:about="http://purl.obolibrary.org/obo/GAZ_00141615">
        <obo:RO_0001025 rdf:resource="http://purl.obolibrary.org/obo/GAZ_00141614"/>
        <obo:IAO_0000115>A rocky island 1.6 km north of Cape Margerie, lying immediately north of Breton Island in the entrance to Port Martin.</obo:IAO_0000115>
        <oboInOwl:hasOBONamespace>GAZ</oboInOwl:hasOBONamespace>
        <oboInOwl:id>GAZ:00141615</oboInOwl:id>
        <rdfs:label>Empereur Island</rdfs:label>
    </owl:NamedIndividual>
    


    <!-- http://purl.obolibrary.org/obo/GAZ_00141616 -->

    <owl:NamedIndividual rdf:about="http://purl.obolibrary.org/obo/GAZ_00141616">
        <obo:RO_0001025 rdf:resource="http://purl.obolibrary.org/obo/GAZ_00141614"/>
        <obo:IAO_0000115>A small rocky island lying 0.2 mi SW of Empereur Island.</obo:IAO_0000115>
        <oboInOwl:hasOBONamespace>GAZ</oboInOwl:hasOBONamespace>
        <oboInOwl:id>GAZ:00141616</oboInOwl:id>
        <rdfs:label>Breton Island</rdfs:label>
    </owl:NamedIndividual>
    


    <!-- http://purl.obolibrary.org/obo/GAZ_00141617 -->

    <owl:NamedIndividual rdf:about="http://purl.obolibrary.org/obo/GAZ_00141617">
        <obo:RO_0001025 rdf:resource="http://purl.obolibrary.org/obo/GAZ_00014089"/>
        <obo:IAO_0000115>A group of about 24 small islands and rocks in Marguerite Bay, the highest 30 m, lying close SW of Emperor Island in the Dion Islands.</obo:IAO_0000115>
        <oboInOwl:hasOBONamespace>GAZ</oboInOwl:hasOBONamespace>
        <oboInOwl:id>GAZ:00141617</oboInOwl:id>
        <rdfs:label>Courtier Islands</rdfs:label>
    </owl:NamedIndividual>
    


    <!-- http://purl.obolibrary.org/obo/GAZ_00141618 -->

    <owl:NamedIndividual rdf:about="http://purl.obolibrary.org/obo/GAZ_00141618">
        <obo:RO_0001025 rdf:resource="http://purl.obolibrary.org/obo/GAZ_00139422"/>
        <obo:IAO_0000115>A group of islands 10 mi NE of William Scoresby Bay.</obo:IAO_0000115>
        <oboInOwl:hasOBONamespace>GAZ</oboInOwl:hasOBONamespace>
        <oboInOwl:id>GAZ:00141618</oboInOwl:id>
        <rdfs:label>Hobbs Islands</rdfs:label>
    </owl:NamedIndividual>
    


    <!-- http://purl.obolibrary.org/obo/GAZ_00141619 -->

    <owl:NamedIndividual rdf:about="http://purl.obolibrary.org/obo/GAZ_00141619">
        <obo:RO_0001025 rdf:resource="http://purl.obolibrary.org/obo/GAZ_00139422"/>
        <obo:IAO_0000115>A group of small islands, the highest rising to 60 m, lying just north of the Hobbs Islands.</obo:IAO_0000115>
        <oboInOwl:hasOBONamespace>GAZ</oboInOwl:hasOBONamespace>
        <oboInOwl:id>GAZ:00141619</oboInOwl:id>
        <rdfs:label>Endresen Islands</rdfs:label>
    </owl:NamedIndividual>
    


    <!-- http://purl.obolibrary.org/obo/GAZ_00141620 -->

    <owl:NamedIndividual rdf:about="http://purl.obolibrary.org/obo/GAZ_00141620">
        <obo:RO_0001025 rdf:resource="http://purl.obolibrary.org/obo/GAZ_00045093"/>
        <obo:IAO_0000115>The second largest island in the Possession Islands, East Antarctica, lying 6 km southwest of Possession Island.</obo:IAO_0000115>
        <oboInOwl:hasOBONamespace>GAZ</oboInOwl:hasOBONamespace>
        <oboInOwl:id>GAZ:00141620</oboInOwl:id>
        <rdfs:label>Foyn Island</rdfs:label>
    </owl:NamedIndividual>
    


    <!-- http://purl.obolibrary.org/obo/GAZ_00141621 -->

    <owl:NamedIndividual rdf:about="http://purl.obolibrary.org/obo/GAZ_00141621">
        <obo:RO_0001025 rdf:resource="http://purl.obolibrary.org/obo/GAZ_00023304"/>
        <obo:IAO_0000115>An island 7 miles long, lying in the Ross Sea about 80 miles east of Cape Hickey, Victoria Land.</obo:IAO_0000115>
        <oboInOwl:hasOBONamespace>GAZ</oboInOwl:hasOBONamespace>
        <oboInOwl:id>GAZ:00141621</oboInOwl:id>
        <rdfs:label>Franklin Island</rdfs:label>
    </owl:NamedIndividual>
    


    <!-- http://purl.obolibrary.org/obo/GAZ_00141622 -->

    <owl:NamedIndividual rdf:about="http://purl.obolibrary.org/obo/GAZ_00141622">
        <obo:RO_0001025 rdf:resource="http://purl.obolibrary.org/obo/GAZ_00141621"/>
        <obo:IAO_0000115>A precipitous cliff forming the south extremity of Franklin Island.</obo:IAO_0000115>
        <oboInOwl:hasOBONamespace>GAZ</oboInOwl:hasOBONamespace>
        <oboInOwl:id>GAZ:00141622</oboInOwl:id>
        <rdfs:label>Bernacchi Head</rdfs:label>
    </owl:NamedIndividual>
    


    <!-- http://purl.obolibrary.org/obo/GAZ_00141623 -->

    <owl:NamedIndividual rdf:about="http://purl.obolibrary.org/obo/GAZ_00141623">
        <obo:RO_0001025 rdf:resource="http://purl.obolibrary.org/obo/GAZ_00023304"/>
        <obo:IAO_0000115>Shoals close to Franklin Island.</obo:IAO_0000115>
        <oboInOwl:hasOBONamespace>GAZ</oboInOwl:hasOBONamespace>
        <oboInOwl:id>GAZ:00141623</oboInOwl:id>
        <rdfs:label>Franklin Shoals</rdfs:label>
    </owl:NamedIndividual>
    


    <!-- http://purl.obolibrary.org/obo/GAZ_00141624 -->

    <owl:NamedIndividual rdf:about="http://purl.obolibrary.org/obo/GAZ_00141624">
        <obo:RO_0001025 rdf:resource="http://purl.obolibrary.org/obo/GAZ_00023304"/>
        <obo:IAO_0000115>An island, 4.8 km long and 555 m high, which projects through the ice of the Koettlitz Glacier just east of Walcott Bay, in Victoria Land.</obo:IAO_0000115>
        <oboInOwl:hasOBONamespace>GAZ</oboInOwl:hasOBONamespace>
        <oboInOwl:id>GAZ:00141624</oboInOwl:id>
        <rdfs:label>Heald Island</rdfs:label>
    </owl:NamedIndividual>
    


    <!-- http://purl.obolibrary.org/obo/GAZ_00141625 -->

    <owl:NamedIndividual rdf:about="http://purl.obolibrary.org/obo/GAZ_00141625">
        <obo:RO_0001025 rdf:resource="http://purl.obolibrary.org/obo/GAZ_00023304"/>
        <obo:IAO_0000115>A bay indenting the coast of Victoria Land between Walcott Glacier and Heald Island.</obo:IAO_0000115>
        <oboInOwl:hasOBONamespace>GAZ</oboInOwl:hasOBONamespace>
        <oboInOwl:id>GAZ:00141625</oboInOwl:id>
        <rdfs:label>Walcott Bay</rdfs:label>
    </owl:NamedIndividual>
    


    <!-- http://purl.obolibrary.org/obo/GAZ_00141626 -->

    <owl:NamedIndividual rdf:about="http://purl.obolibrary.org/obo/GAZ_00141626">
        <obo:RO_0001025 rdf:resource="http://purl.obolibrary.org/obo/GAZ_00023352"/>
        <obo:IAO_0000115>A low rocky island (0.3 km southeast of Helene Island at the west end of Geologie Archipelago.</obo:IAO_0000115>
        <oboInOwl:hasOBONamespace>GAZ</oboInOwl:hasOBONamespace>
        <oboInOwl:id>GAZ:00141626</oboInOwl:id>
        <rdfs:label>Ifo Island</rdfs:label>
    </owl:NamedIndividual>
    


    <!-- http://purl.obolibrary.org/obo/GAZ_00141627 -->

    <owl:NamedIndividual rdf:about="http://purl.obolibrary.org/obo/GAZ_00141627">
        <obo:RO_0001025 rdf:resource="http://purl.obolibrary.org/obo/GAZ_00023352"/>
        <obo:IAO_0000115>An isolated rock dome, 27 m, which protrudes through the ice in NW Rostand Island in the Geologie Archipelago.</obo:IAO_0000115>
        <oboInOwl:hasOBONamespace>GAZ</oboInOwl:hasOBONamespace>
        <oboInOwl:id>GAZ:00141627</oboInOwl:id>
        <rdfs:label>Tour de Pise</rdfs:label>
    </owl:NamedIndividual>
    


    <!-- http://purl.obolibrary.org/obo/GAZ_00141628 -->

    <owl:NamedIndividual rdf:about="http://purl.obolibrary.org/obo/GAZ_00141628">
        <obo:RO_0001025 rdf:resource="http://purl.obolibrary.org/obo/GAZ_00023352"/>
        <obo:IAO_0000115>A small rocky island 0.05 mi W of the N end of Carrel Island in the Geologie Archipelago.</obo:IAO_0000115>
        <oboInOwl:hasOBONamespace>GAZ</oboInOwl:hasOBONamespace>
        <oboInOwl:id>GAZ:00141628</oboInOwl:id>
        <rdfs:label>Maregraphe Island</rdfs:label>
    </owl:NamedIndividual>
    


    <!-- http://purl.obolibrary.org/obo/GAZ_00141629 -->

    <owl:NamedIndividual rdf:about="http://purl.obolibrary.org/obo/GAZ_00141629">
        <obo:RO_0001025 rdf:resource="http://purl.obolibrary.org/obo/GAZ_00023352"/>
        <obo:IAO_0000115>A rocky island 0.25 mi long lying 0.1 mi S of Petrel Island in the Geologie Archipelago.</obo:IAO_0000115>
        <oboInOwl:hasOBONamespace>GAZ</oboInOwl:hasOBONamespace>
        <oboInOwl:id>GAZ:00141629</oboInOwl:id>
        <rdfs:label>Carrel Island</rdfs:label>
    </owl:NamedIndividual>
    


    <!-- http://purl.obolibrary.org/obo/GAZ_00141630 -->

    <owl:NamedIndividual rdf:about="http://purl.obolibrary.org/obo/GAZ_00141630">
        <obo:RO_0001025 rdf:resource="http://purl.obolibrary.org/obo/GAZ_00023352"/>
        <obo:IAO_0000115>A rocky island 0.2 mi long, 0.1 mi SE of Petrel Island in the Geologie Archipelago.</obo:IAO_0000115>
        <oboInOwl:hasOBONamespace>GAZ</oboInOwl:hasOBONamespace>
        <oboInOwl:id>GAZ:00141630</oboInOwl:id>
        <rdfs:label>Rostand Island</rdfs:label>
    </owl:NamedIndividual>
    


    <!-- http://purl.obolibrary.org/obo/GAZ_00141631 -->

    <owl:NamedIndividual rdf:about="http://purl.obolibrary.org/obo/GAZ_00141631">
        <obo:RO_0001025 rdf:resource="http://purl.obolibrary.org/obo/GAZ_00023352"/>
        <obo:IAO_0000115>A small group of rocky islands at the NE end of the Geologie Archipelago, 2.5 mi N of Astrolabe Glacier Tongue.</obo:IAO_0000115>
        <oboInOwl:hasOBONamespace>GAZ</oboInOwl:hasOBONamespace>
        <oboInOwl:id>GAZ:00141631</oboInOwl:id>
        <rdfs:label>Dumoulin Islands</rdfs:label>
    </owl:NamedIndividual>
    


    <!-- http://purl.obolibrary.org/obo/GAZ_00141632 -->

    <owl:NamedIndividual rdf:about="http://purl.obolibrary.org/obo/GAZ_00141632">
        <obo:RO_0001025 rdf:resource="http://purl.obolibrary.org/obo/GAZ_00023304"/>
        <obo:IAO_0000115>A bay about 13 mi wide between Cape Evans and Hut Point Peninsula, on the W side of Ross Island.</obo:IAO_0000115>
        <oboInOwl:hasOBONamespace>GAZ</oboInOwl:hasOBONamespace>
        <oboInOwl:id>GAZ:00141632</oboInOwl:id>
        <rdfs:label>Erebus Bay</rdfs:label>
    </owl:NamedIndividual>
    


    <!-- http://purl.obolibrary.org/obo/GAZ_00141633 -->

    <owl:NamedIndividual rdf:about="http://purl.obolibrary.org/obo/GAZ_00141633">
        <obo:RO_0001025 rdf:resource="http://purl.obolibrary.org/obo/GAZ_00023294"/>
        <obo:IAO_0000115>An island lying 2.4 km west of Langhovde-kita Point in the east part of Lutzow-Holm Bay.</obo:IAO_0000115>
        <oboInOwl:hasOBONamespace>GAZ</oboInOwl:hasOBONamespace>
        <oboInOwl:id>GAZ:00141633</oboInOwl:id>
        <rdfs:label>Indrehovdeholmen</rdfs:label>
    </owl:NamedIndividual>
    


    <!-- http://purl.obolibrary.org/obo/GAZ_00141634 -->

    <owl:NamedIndividual rdf:about="http://purl.obolibrary.org/obo/GAZ_00141634">
        <obo:RO_0001025 rdf:resource="http://purl.obolibrary.org/obo/GAZ_00139422"/>
        <obo:IAO_0000115>A group of small islands lying immediately off Cape Boothby, Enderby Land.</obo:IAO_0000115>
        <oboInOwl:hasOBONamespace>GAZ</oboInOwl:hasOBONamespace>
        <oboInOwl:id>GAZ:00141634</oboInOwl:id>
        <rdfs:label>Jagar Islands</rdfs:label>
    </owl:NamedIndividual>
    


    <!-- http://purl.obolibrary.org/obo/GAZ_00141635 -->

    <owl:NamedIndividual rdf:about="http://purl.obolibrary.org/obo/GAZ_00141635">
        <obo:RO_0001025 rdf:resource="http://purl.obolibrary.org/obo/GAZ_00139422"/>
        <obo:IAO_0000115>An island 0.8 km long, lying 24 km north-northeast of Byrd Head.</obo:IAO_0000115>
        <oboInOwl:hasOBONamespace>GAZ</oboInOwl:hasOBONamespace>
        <oboInOwl:id>GAZ:00141635</oboInOwl:id>
        <rdfs:label>Kidson Island</rdfs:label>
    </owl:NamedIndividual>
    


    <!-- http://purl.obolibrary.org/obo/GAZ_00141636 -->

    <owl:NamedIndividual rdf:about="http://purl.obolibrary.org/obo/GAZ_00141636">
        <obo:RO_0001025 rdf:resource="http://purl.obolibrary.org/obo/GAZ_00141480"/>
        <obo:IAO_0000115>An island 2.5 mi long, lying off the south shore of James Ross Island in the SW entrance to Admiralty Sound in Antarctica.</obo:IAO_0000115>
        <oboInOwl:hasOBONamespace>GAZ</oboInOwl:hasOBONamespace>
        <oboInOwl:id>GAZ:00141636</oboInOwl:id>
        <rdfs:label>Lockyer Island</rdfs:label>
    </owl:NamedIndividual>
    


    <!-- http://purl.obolibrary.org/obo/GAZ_00141637 -->

    <owl:NamedIndividual rdf:about="http://purl.obolibrary.org/obo/GAZ_00141637">
        <obo:RO_0001025 rdf:resource="http://purl.obolibrary.org/obo/GAZ_00141556"/>
        <obo:IAO_0000115>A small horseshoe-shaped island which has numerous areas of exposed rock, lying 13 km north of the northwest end of Siple Island, off the coast of Marie Byrd Land.</obo:IAO_0000115>
        <oboInOwl:hasOBONamespace>GAZ</oboInOwl:hasOBONamespace>
        <oboInOwl:id>GAZ:00141637</oboInOwl:id>
        <rdfs:label>Maher Island</rdfs:label>
    </owl:NamedIndividual>
    


    <!-- http://purl.obolibrary.org/obo/GAZ_00141638 -->

    <owl:NamedIndividual rdf:about="http://purl.obolibrary.org/obo/GAZ_00141638">
        <obo:RO_0001025 rdf:resource="http://purl.obolibrary.org/obo/GAZ_00051500"/>
        <obo:IAO_0000115>An archipelago of two islands lying close west of the Thala Hills, off the coast of Enderby Land.</obo:IAO_0000115>
        <oboInOwl:hasOBONamespace>GAZ</oboInOwl:hasOBONamespace>
        <oboInOwl:id>GAZ:00141638</oboInOwl:id>
        <rdfs:label>Myall Islands</rdfs:label>
    </owl:NamedIndividual>
    


    <!-- http://purl.obolibrary.org/obo/GAZ_00141639 -->

    <owl:NamedIndividual rdf:about="http://purl.obolibrary.org/obo/GAZ_00141639">
        <obo:RO_0001025 rdf:resource="http://purl.obolibrary.org/obo/GAZ_00141297"/>
        <obo:IAO_0000115>A small ice-covered island lying close to Siple Island in the west extremity of Russell Bay, off the coast of Marie Byrd Land.</obo:IAO_0000115>
        <oboInOwl:hasOBONamespace>GAZ</oboInOwl:hasOBONamespace>
        <oboInOwl:id>GAZ:00141639</oboInOwl:id>
        <rdfs:label>Pranke Island</rdfs:label>
    </owl:NamedIndividual>
    


    <!-- http://purl.obolibrary.org/obo/GAZ_00141640 -->

    <owl:NamedIndividual rdf:about="http://purl.obolibrary.org/obo/GAZ_00141640">
        <obo:RO_0001025 rdf:resource="http://purl.obolibrary.org/obo/GAZ_00141484"/>
        <obo:IAO_0000115>The largest of the Henkes Islands, lying off the south end of Adelaide Island.</obo:IAO_0000115>
        <oboInOwl:hasOBONamespace>GAZ</oboInOwl:hasOBONamespace>
        <oboInOwl:id>GAZ:00141640</oboInOwl:id>
        <rdfs:label>Preston Island</rdfs:label>
    </owl:NamedIndividual>
    


    <!-- http://purl.obolibrary.org/obo/GAZ_00141641 -->

    <owl:NamedIndividual rdf:about="http://purl.obolibrary.org/obo/GAZ_00141641">
        <obo:RO_0001025 rdf:resource="http://purl.obolibrary.org/obo/GAZ_00051499"/>
        <obo:IAO_0000115>An island 1.9 km long, lying just east of Lamplugh Island, off the coast of Victoria Land.</obo:IAO_0000115>
        <oboInOwl:hasOBONamespace>GAZ</oboInOwl:hasOBONamespace>
        <oboInOwl:id>GAZ:00141641</oboInOwl:id>
        <rdfs:label>Prior Island</rdfs:label>
    </owl:NamedIndividual>
    


    <!-- http://purl.obolibrary.org/obo/GAZ_00141642 -->

    <owl:NamedIndividual rdf:about="http://purl.obolibrary.org/obo/GAZ_00141642">
        <obo:RO_0001025 rdf:resource="http://purl.obolibrary.org/obo/GAZ_00141643"/>
        <obo:IAO_0000115>An ice-covered island 22 km long in the Marshall Archipelago. It lies 6 km east of Cronenwett Island in the western part of Sulzberger Ice Shelf.</obo:IAO_0000115>
        <oboInOwl:hasOBONamespace>GAZ</oboInOwl:hasOBONamespace>
        <oboInOwl:id>GAZ:00141642</oboInOwl:id>
        <rdfs:label>Przybyszewski Island</rdfs:label>
    </owl:NamedIndividual>
    


    <!-- http://purl.obolibrary.org/obo/GAZ_00141643 -->

    <owl:NamedIndividual rdf:about="http://purl.obolibrary.org/obo/GAZ_00141643">
        <obo:RO_0001025 rdf:resource="http://purl.obolibrary.org/obo/GAZ_00139775"/>
        <obo:IAO_0000115>An extensive group of large ice-covered islands within Sulzberger Ice Shelf.</obo:IAO_0000115>
        <oboInOwl:hasOBONamespace>GAZ</oboInOwl:hasOBONamespace>
        <oboInOwl:id>GAZ:00141643</oboInOwl:id>
        <rdfs:label>Marshall Archipelago</rdfs:label>
    </owl:NamedIndividual>
    


    <!-- http://purl.obolibrary.org/obo/GAZ_00141644 -->

    <owl:NamedIndividual rdf:about="http://purl.obolibrary.org/obo/GAZ_00141644">
        <obo:RO_0001025 rdf:resource="http://purl.obolibrary.org/obo/GAZ_00141643"/>
        <obo:IAO_0000115>A high, ice-covered island about 20 mi long. It lies between Vollmer Island and Steventon Island in the Marshall Archipelago, off the coast of Marie Byrd Land.</obo:IAO_0000115>
        <oboInOwl:hasOBONamespace>GAZ</oboInOwl:hasOBONamespace>
        <oboInOwl:id>GAZ:00141644</oboInOwl:id>
        <rdfs:label>Cronenwett Island</rdfs:label>
    </owl:NamedIndividual>
    


    <!-- http://purl.obolibrary.org/obo/GAZ_00141645 -->

    <owl:NamedIndividual rdf:about="http://purl.obolibrary.org/obo/GAZ_00141645">
        <obo:RO_0001025 rdf:resource="http://purl.obolibrary.org/obo/GAZ_00141643"/>
        <obo:IAO_0000115>A broad ice-covered island about 24 mi long, lying W of Court Ridge in the Sulzberger Ice Shelf.</obo:IAO_0000115>
        <oboInOwl:hasOBONamespace>GAZ</oboInOwl:hasOBONamespace>
        <oboInOwl:id>GAZ:00141645</oboInOwl:id>
        <rdfs:label>Steventon Island</rdfs:label>
    </owl:NamedIndividual>
    


    <!-- http://purl.obolibrary.org/obo/GAZ_00141646 -->

    <owl:NamedIndividual rdf:about="http://purl.obolibrary.org/obo/GAZ_00141646">
        <obo:RO_0001025 rdf:resource="http://purl.obolibrary.org/obo/GAZ_00141642"/>
        <obo:IAO_0000115>A rock outcrop in the S part of Przybyszewski Island in the Marshall Archipelago.</obo:IAO_0000115>
        <oboInOwl:hasOBONamespace>GAZ</oboInOwl:hasOBONamespace>
        <oboInOwl:id>GAZ:00141646</oboInOwl:id>
        <rdfs:label>Barela Rock</rdfs:label>
    </owl:NamedIndividual>
    


    <!-- http://purl.obolibrary.org/obo/GAZ_00141647 -->

    <owl:NamedIndividual rdf:about="http://purl.obolibrary.org/obo/GAZ_00141647">
        <obo:RO_0001025 rdf:resource="http://purl.obolibrary.org/obo/GAZ_00141643"/>
        <obo:IAO_0000115>One of the ice-covered islands in Marshall Archipelago, located within Sulzberger Ice Shelf, coastal Marie Byrd Land.</obo:IAO_0000115>
        <oboInOwl:hasOBONamespace>GAZ</oboInOwl:hasOBONamespace>
        <oboInOwl:id>GAZ:00141647</oboInOwl:id>
        <rdfs:label>Gould Island</rdfs:label>
    </owl:NamedIndividual>
    


    <!-- http://purl.obolibrary.org/obo/GAZ_00141648 -->

    <owl:NamedIndividual rdf:about="http://purl.obolibrary.org/obo/GAZ_00141648">
        <obo:RO_0001025 rdf:resource="http://purl.obolibrary.org/obo/GAZ_00141643"/>
        <obo:IAO_0000115>An ice-covered island surmounted by several peaks, lying 6 mi W of Saunders Mountain in the E part of Sulzberger Ice Shelf.</obo:IAO_0000115>
        <oboInOwl:hasOBONamespace>GAZ</oboInOwl:hasOBONamespace>
        <oboInOwl:id>GAZ:00141648</oboInOwl:id>
        <rdfs:label>Radford Island</rdfs:label>
    </owl:NamedIndividual>
    


    <!-- http://purl.obolibrary.org/obo/GAZ_00141649 -->

    <owl:NamedIndividual rdf:about="http://purl.obolibrary.org/obo/GAZ_00141649">
        <obo:RO_0001025 rdf:resource="http://purl.obolibrary.org/obo/GAZ_00141643"/>
        <obo:IAO_0000115>An ice-covered island about 4 mi long, lying 5 mi NW of Nolan Island in Marshall Archipelago.</obo:IAO_0000115>
        <oboInOwl:hasOBONamespace>GAZ</oboInOwl:hasOBONamespace>
        <oboInOwl:id>GAZ:00141649</oboInOwl:id>
        <rdfs:label>Benton Island</rdfs:label>
    </owl:NamedIndividual>
    


    <!-- http://purl.obolibrary.org/obo/GAZ_00141650 -->

    <owl:NamedIndividual rdf:about="http://purl.obolibrary.org/obo/GAZ_00141650">
        <obo:RO_0001025 rdf:resource="http://purl.obolibrary.org/obo/GAZ_00141643"/>
        <obo:IAO_0000115>One of the ice-covered islands in Marshall Archipelago, located within Sulzberger Ice Shelf, coastal Marie Byrd Land. The island is 7 mi long and 1 mi wide and lies 13 mi SW of Steventon Island.</obo:IAO_0000115>
        <oboInOwl:hasOBONamespace>GAZ</oboInOwl:hasOBONamespace>
        <oboInOwl:id>GAZ:00141650</oboInOwl:id>
        <rdfs:label>Grinder Island</rdfs:label>
    </owl:NamedIndividual>
    


    <!-- http://purl.obolibrary.org/obo/GAZ_00141651 -->

    <owl:NamedIndividual rdf:about="http://purl.obolibrary.org/obo/GAZ_00141651">
        <obo:RO_0001025 rdf:resource="http://purl.obolibrary.org/obo/GAZ_00141643"/>
        <obo:IAO_0000115>An ice-covered island 6 mi long, lying 2 mi N of Court Ridge in Sulzberger Ice Shelf, along the coast of Marie Byrd Land.</obo:IAO_0000115>
        <oboInOwl:hasOBONamespace>GAZ</oboInOwl:hasOBONamespace>
        <oboInOwl:id>GAZ:00141651</oboInOwl:id>
        <rdfs:label>Nolan Island</rdfs:label>
    </owl:NamedIndividual>
    


    <!-- http://purl.obolibrary.org/obo/GAZ_00141652 -->

    <owl:NamedIndividual rdf:about="http://purl.obolibrary.org/obo/GAZ_00141652">
        <obo:RO_0001025 rdf:resource="http://purl.obolibrary.org/obo/GAZ_00141648"/>
        <obo:IAO_0000115>An ice-covered knoll 4 mi SW of Mount Dane in the W part of Radford Island, Marshall Archipelago.</obo:IAO_0000115>
        <oboInOwl:hasOBONamespace>GAZ</oboInOwl:hasOBONamespace>
        <oboInOwl:id>GAZ:00141652</oboInOwl:id>
        <rdfs:label>Clark Knoll</rdfs:label>
    </owl:NamedIndividual>
    


    <!-- http://purl.obolibrary.org/obo/GAZ_00141653 -->

    <owl:NamedIndividual rdf:about="http://purl.obolibrary.org/obo/GAZ_00141653">
        <obo:RO_0001025 rdf:resource="http://purl.obolibrary.org/obo/GAZ_00141643"/>
        <obo:IAO_0000115>An ice-covered island 10 mi long, between Kizer and Steventon Islands in the Sulzberger Ice Shelf.</obo:IAO_0000115>
        <oboInOwl:hasOBONamespace>GAZ</oboInOwl:hasOBONamespace>
        <oboInOwl:id>GAZ:00141653</oboInOwl:id>
        <rdfs:label>Moody Island</rdfs:label>
    </owl:NamedIndividual>
    


    <!-- http://purl.obolibrary.org/obo/GAZ_00141654 -->

    <owl:NamedIndividual rdf:about="http://purl.obolibrary.org/obo/GAZ_00141654">
        <obo:RO_0001025 rdf:resource="http://purl.obolibrary.org/obo/GAZ_00141643"/>
        <obo:IAO_0000115>An ice-covered island 5 mi long, lying 3 mi SW of Grinder Island in Marshall Archipelago, off the coast of Marie Byrd Land.</obo:IAO_0000115>
        <oboInOwl:hasOBONamespace>GAZ</oboInOwl:hasOBONamespace>
        <oboInOwl:id>GAZ:00141654</oboInOwl:id>
        <rdfs:label>Orr Island</rdfs:label>
    </owl:NamedIndividual>
    


    <!-- http://purl.obolibrary.org/obo/GAZ_00141655 -->

    <owl:NamedIndividual rdf:about="http://purl.obolibrary.org/obo/GAZ_00141655">
        <obo:RO_0001025 rdf:resource="http://purl.obolibrary.org/obo/GAZ_00141643"/>
        <obo:IAO_0000115>An ice-covered island, 2 mi long, in Marshall Archipelago. It lies between Nolan Island and Court Ridge in Sulzberger Ice Shelf.</obo:IAO_0000115>
        <oboInOwl:hasOBONamespace>GAZ</oboInOwl:hasOBONamespace>
        <oboInOwl:id>GAZ:00141655</oboInOwl:id>
        <rdfs:label>Kramer Island</rdfs:label>
    </owl:NamedIndividual>
    


    <!-- http://purl.obolibrary.org/obo/GAZ_00141656 -->

    <owl:NamedIndividual rdf:about="http://purl.obolibrary.org/obo/GAZ_00141656">
        <obo:RO_0001025 rdf:resource="http://purl.obolibrary.org/obo/GAZ_00141643"/>
        <obo:IAO_0000115>An ice-covered island in Marshall Archipelago, lying between Hutchinson Island and Guest Peninsula within Sulzberger Ice Shelf.</obo:IAO_0000115>
        <oboInOwl:hasOBONamespace>GAZ</oboInOwl:hasOBONamespace>
        <oboInOwl:id>GAZ:00141656</oboInOwl:id>
        <rdfs:label>Hannah Island</rdfs:label>
    </owl:NamedIndividual>
    


    <!-- http://purl.obolibrary.org/obo/GAZ_00141657 -->

    <owl:NamedIndividual rdf:about="http://purl.obolibrary.org/obo/GAZ_00141657">
        <obo:RO_0001025 rdf:resource="http://purl.obolibrary.org/obo/GAZ_00141643"/>
        <obo:IAO_0000115>An ice-covered island about 15 mi long, lying 10 mi SW of Cronenwett Island at the W end of Sulzberger Ice Shelf.</obo:IAO_0000115>
        <oboInOwl:hasOBONamespace>GAZ</oboInOwl:hasOBONamespace>
        <oboInOwl:id>GAZ:00141657</oboInOwl:id>
        <rdfs:label>Kizer Island</rdfs:label>
    </owl:NamedIndividual>
    


    <!-- http://purl.obolibrary.org/obo/GAZ_00141658 -->

    <owl:NamedIndividual rdf:about="http://purl.obolibrary.org/obo/GAZ_00141658">
        <obo:RO_0001025 rdf:resource="http://purl.obolibrary.org/obo/GAZ_00141643"/>
        <obo:IAO_0000115>An ice-covered island 15 mi long, lying 10 mi E of Vollmer Island in Marshall Archipelago.</obo:IAO_0000115>
        <oboInOwl:hasOBONamespace>GAZ</oboInOwl:hasOBONamespace>
        <oboInOwl:id>GAZ:00141658</oboInOwl:id>
        <rdfs:label>Hutchinson Island</rdfs:label>
    </owl:NamedIndividual>
    


    <!-- http://purl.obolibrary.org/obo/GAZ_00141659 -->

    <owl:NamedIndividual rdf:about="http://purl.obolibrary.org/obo/GAZ_00141659">
        <obo:RO_0001025 rdf:resource="http://purl.obolibrary.org/obo/GAZ_00141643"/>
        <obo:IAO_0000115>An ice-covered island, 4 mi long, in Marshall Archipelago. It lies between Moody Island and Grinder Island in Sulzberger Ice Shelf.</obo:IAO_0000115>
        <oboInOwl:hasOBONamespace>GAZ</oboInOwl:hasOBONamespace>
        <oboInOwl:id>GAZ:00141659</oboInOwl:id>
        <rdfs:label>Madden Island</rdfs:label>
    </owl:NamedIndividual>
    


    <!-- http://purl.obolibrary.org/obo/GAZ_00141660 -->

    <owl:NamedIndividual rdf:about="http://purl.obolibrary.org/obo/GAZ_00141660">
        <obo:RO_0001025 rdf:resource="http://purl.obolibrary.org/obo/GAZ_00141643"/>
        <obo:IAO_0000115>A small ice-covered island in Sulzherger Ice Shelf, located 1 mi NW of Benton Island and 5 mi E of Przybyszewski Island in Marshall Archipelago.</obo:IAO_0000115>
        <oboInOwl:hasOBONamespace>GAZ</oboInOwl:hasOBONamespace>
        <oboInOwl:id>GAZ:00141660</oboInOwl:id>
        <rdfs:label>Thode Island</rdfs:label>
    </owl:NamedIndividual>
    


    <!-- http://purl.obolibrary.org/obo/GAZ_00141661 -->

    <owl:NamedIndividual rdf:about="http://purl.obolibrary.org/obo/GAZ_00141661">
        <obo:RO_0001025 rdf:resource="http://purl.obolibrary.org/obo/GAZ_00141643"/>
        <obo:IAO_0000115>A small ice-covered island in Marshall Archipelago, lying 2 mi off the NE part of Steventon Island within Sulzberger Ice Shelf.</obo:IAO_0000115>
        <oboInOwl:hasOBONamespace>GAZ</oboInOwl:hasOBONamespace>
        <oboInOwl:id>GAZ:00141661</oboInOwl:id>
        <rdfs:label>Spencer Island</rdfs:label>
    </owl:NamedIndividual>
    


    <!-- http://purl.obolibrary.org/obo/GAZ_00141662 -->

    <owl:NamedIndividual rdf:about="http://purl.obolibrary.org/obo/GAZ_00141662">
        <obo:RO_0001025 rdf:resource="http://purl.obolibrary.org/obo/GAZ_00014089"/>
        <obo:IAO_0000115>A scattered group of small, low, mainly ice-covered islands and rocks which extend about 18 km in a NE-SW direction, lying in southern Marguerite Bay off the west coast of Antarctic Peninsula.</obo:IAO_0000115>
        <oboInOwl:hasOBONamespace>GAZ</oboInOwl:hasOBONamespace>
        <oboInOwl:id>GAZ:00141662</oboInOwl:id>
        <rdfs:label>Puffball Islands</rdfs:label>
    </owl:NamedIndividual>
    


    <!-- http://purl.obolibrary.org/obo/GAZ_00141663 -->

    <owl:NamedIndividual rdf:about="http://purl.obolibrary.org/obo/GAZ_00141663">
        <obo:RO_0001025 rdf:resource="http://purl.obolibrary.org/obo/GAZ_00139960"/>
        <obo:IAO_0000115>A prominent rocky island lying between the foot of Clarke Glacier and Keyhole Island on the south side of Mikkelsen Bay, off the west coast of Graham Land.</obo:IAO_0000115>
        <oboInOwl:hasOBONamespace>GAZ</oboInOwl:hasOBONamespace>
        <oboInOwl:id>GAZ:00141663</oboInOwl:id>
        <rdfs:label>Query Island</rdfs:label>
    </owl:NamedIndividual>
    


    <!-- http://purl.obolibrary.org/obo/GAZ_00141664 -->

    <owl:NamedIndividual rdf:about="http://purl.obolibrary.org/obo/GAZ_00141664">
        <obo:RO_0001025 rdf:resource="http://purl.obolibrary.org/obo/GAZ_00139422"/>
        <obo:IAO_0000115>A small coastal island 4.8 km east of Cape Daly.</obo:IAO_0000115>
        <oboInOwl:hasOBONamespace>GAZ</oboInOwl:hasOBONamespace>
        <oboInOwl:id>GAZ:00141664</oboInOwl:id>
        <rdfs:label>Safety Island</rdfs:label>
    </owl:NamedIndividual>
    


    <!-- http://purl.obolibrary.org/obo/GAZ_00141665 -->

    <owl:NamedIndividual rdf:about="http://purl.obolibrary.org/obo/GAZ_00141665">
        <obo:RO_0001025 rdf:resource="http://purl.obolibrary.org/obo/GAZ_00141552"/>
        <obo:IAO_0000115>A group of islands extending west from Black Head, off the west coast of Graham Land.</obo:IAO_0000115>
        <oboInOwl:hasOBONamespace>GAZ</oboInOwl:hasOBONamespace>
        <oboInOwl:id>GAZ:00141665</oboInOwl:id>
        <rdfs:label>Saffery Islands</rdfs:label>
    </owl:NamedIndividual>
    


    <!-- http://purl.obolibrary.org/obo/GAZ_00141666 -->

    <owl:NamedIndividual rdf:about="http://purl.obolibrary.org/obo/GAZ_00141666">
        <obo:RO_0001025 rdf:resource="http://purl.obolibrary.org/obo/GAZ_00141555"/>
        <obo:IAO_0000115>A group of four islands lying 3.2 km north of the central part of McKinnon Island, off the coast of Enderby Land.</obo:IAO_0000115>
        <oboInOwl:hasOBONamespace>GAZ</oboInOwl:hasOBONamespace>
        <oboInOwl:id>GAZ:00141666</oboInOwl:id>
        <rdfs:label>Shaw Islands</rdfs:label>
    </owl:NamedIndividual>
    


    <!-- http://purl.obolibrary.org/obo/GAZ_00141667 -->

    <owl:NamedIndividual rdf:about="http://purl.obolibrary.org/obo/GAZ_00141667">
        <obo:RO_0001025 rdf:resource="http://purl.obolibrary.org/obo/GAZ_00139422"/>
        <obo:IAO_0000115>A group of small islands lying at the southeast side of Islay in the William Scoresby Archipelago.</obo:IAO_0000115>
        <oboInOwl:hasOBONamespace>GAZ</oboInOwl:hasOBONamespace>
        <oboInOwl:id>GAZ:00141667</oboInOwl:id>
        <rdfs:label>Sheehan Islands</rdfs:label>
    </owl:NamedIndividual>
    


    <!-- http://purl.obolibrary.org/obo/GAZ_00141668 -->

    <owl:NamedIndividual rdf:about="http://purl.obolibrary.org/obo/GAZ_00141668">
        <obo:RO_0001025 rdf:resource="http://purl.obolibrary.org/obo/GAZ_00023294"/>
        <obo:IAO_0000115>Two islands lying in the east part of Lutzow-Holm Bay, 6 km west of Langhovde-kita Point.</obo:IAO_0000115>
        <oboInOwl:hasOBONamespace>GAZ</oboInOwl:hasOBONamespace>
        <oboInOwl:id>GAZ:00141668</oboInOwl:id>
        <rdfs:label>Sigaren Islands</rdfs:label>
    </owl:NamedIndividual>
    


    <!-- http://purl.obolibrary.org/obo/GAZ_00141669 -->

    <owl:NamedIndividual rdf:about="http://purl.obolibrary.org/obo/GAZ_00141669">
        <rdf:type rdf:resource="http://purl.obolibrary.org/obo/ENVO_00000305"/>
        <obo:RO_0001025 rdf:resource="http://purl.obolibrary.org/obo/GAZ_00023301"/>
        <obo:IAO_0000115>A cape forming the northern extremity of Adelaide Island.</obo:IAO_0000115>
        <oboInOwl:hasOBONamespace>GAZ</oboInOwl:hasOBONamespace>
        <oboInOwl:id>GAZ:00141669</oboInOwl:id>
        <rdfs:label>Cape Mascart</rdfs:label>
    </owl:NamedIndividual>
    


    <!-- http://purl.obolibrary.org/obo/GAZ_00141670 -->

    <owl:NamedIndividual rdf:about="http://purl.obolibrary.org/obo/GAZ_00141670">
        <obo:RO_0001025 rdf:resource="http://purl.obolibrary.org/obo/GAZ_00014089"/>
        <obo:IAO_0000115>A group of small ice-covered islands lying close to Cape Mascart, the northeast extremity of Adelaide Island.</obo:IAO_0000115>
        <oboInOwl:hasOBONamespace>GAZ</oboInOwl:hasOBONamespace>
        <oboInOwl:id>GAZ:00141670</oboInOwl:id>
        <rdfs:label>Sillard Islands</rdfs:label>
    </owl:NamedIndividual>
    


    <!-- http://purl.obolibrary.org/obo/GAZ_00141671 -->

    <owl:NamedIndividual rdf:about="http://purl.obolibrary.org/obo/GAZ_00141671">
        <obo:RO_0001025 rdf:resource="http://purl.obolibrary.org/obo/GAZ_00139422"/>
        <obo:IAO_0000115>A bay, 1 mi long, indenting the seaward end of Breidnes Peninsula, Vestfold Hills, just S of Davis Station.</obo:IAO_0000115>
        <oboInOwl:hasOBONamespace>GAZ</oboInOwl:hasOBONamespace>
        <oboInOwl:id>GAZ:00141671</oboInOwl:id>
        <rdfs:label>Heidemann Bay</rdfs:label>
    </owl:NamedIndividual>
    


    <!-- http://purl.obolibrary.org/obo/GAZ_00141672 -->

    <owl:NamedIndividual rdf:about="http://purl.obolibrary.org/obo/GAZ_00141672">
        <obo:RO_0001025 rdf:resource="http://purl.obolibrary.org/obo/GAZ_00139422"/>
        <obo:IAO_0000115>A small island off the Vestfold Hills, lying 0.8 km southwest of the south entrance point to Heidemann Bay.</obo:IAO_0000115>
        <oboInOwl:hasOBONamespace>GAZ</oboInOwl:hasOBONamespace>
        <oboInOwl:id>GAZ:00141672</oboInOwl:id>
        <rdfs:label>Suter Island</rdfs:label>
    </owl:NamedIndividual>
    


    <!-- http://purl.obolibrary.org/obo/GAZ_00141673 -->

    <owl:NamedIndividual rdf:about="http://purl.obolibrary.org/obo/GAZ_00141673">
        <obo:RO_0001025 rdf:resource="http://purl.obolibrary.org/obo/GAZ_00023294"/>
        <obo:IAO_0000115>A group of three small islands lying 8 km west of Hamnenabben Head in the east part of Lutzow-Holm Bay.</obo:IAO_0000115>
        <oboInOwl:hasOBONamespace>GAZ</oboInOwl:hasOBONamespace>
        <oboInOwl:id>GAZ:00141673</oboInOwl:id>
        <rdfs:label>Systerflesene Islands</rdfs:label>
    </owl:NamedIndividual>
    


    <!-- http://purl.obolibrary.org/obo/GAZ_00141674 -->

    <owl:NamedIndividual rdf:about="http://purl.obolibrary.org/obo/GAZ_00141674">
        <obo:RO_0001025 rdf:resource="http://purl.obolibrary.org/obo/GAZ_00051499"/>
        <obo:IAO_0000115>A small rocky island 1.1 km east of Tristan Island and 0.6 km north of the east point on Cape Jules.</obo:IAO_0000115>
        <oboInOwl:hasOBONamespace>GAZ</oboInOwl:hasOBONamespace>
        <oboInOwl:id>GAZ:00141674</oboInOwl:id>
        <rdfs:label>Yseult Island</rdfs:label>
    </owl:NamedIndividual>
    


    <!-- http://purl.obolibrary.org/obo/GAZ_00141675 -->

    <owl:NamedIndividual rdf:about="http://purl.obolibrary.org/obo/GAZ_00141675">
        <obo:RO_0001025 rdf:resource="http://purl.obolibrary.org/obo/GAZ_00051499"/>
        <obo:IAO_0000115>A small rocky island 1.1 km west of Yseult Island and 0.3 km north of the west point on Cape Jules.</obo:IAO_0000115>
        <oboInOwl:hasOBONamespace>GAZ</oboInOwl:hasOBONamespace>
        <oboInOwl:id>GAZ:00141675</oboInOwl:id>
        <rdfs:label>Tristan Island</rdfs:label>
    </owl:NamedIndividual>
    


    <!-- http://purl.obolibrary.org/obo/GAZ_00141676 -->

    <owl:NamedIndividual rdf:about="http://purl.obolibrary.org/obo/GAZ_00141676">
        <obo:RO_0001025 rdf:resource="http://purl.obolibrary.org/obo/GAZ_00139422"/>
        <obo:IAO_0000115>A steep-sided, isolated island lying 6 km northeast of Tilley Nunatak, off the coast of Mac Robertson Land.</obo:IAO_0000115>
        <oboInOwl:hasOBONamespace>GAZ</oboInOwl:hasOBONamespace>
        <oboInOwl:id>GAZ:00141676</oboInOwl:id>
        <rdfs:label>Uksen Island</rdfs:label>
    </owl:NamedIndividual>
    


    <!-- http://purl.obolibrary.org/obo/GAZ_00141677 -->

    <owl:NamedIndividual rdf:about="http://purl.obolibrary.org/obo/GAZ_00141677">
        <obo:RO_0001025 rdf:resource="http://purl.obolibrary.org/obo/GAZ_00140392"/>
        <obo:IAO_0000115>A rocky island, 1.5 mi long, lying 2 mi off the W side of Alexander Island in Lazarev Bay.</obo:IAO_0000115>
        <oboInOwl:hasOBONamespace>GAZ</oboInOwl:hasOBONamespace>
        <oboInOwl:id>GAZ:00141677</oboInOwl:id>
        <rdfs:label>Dint Island</rdfs:label>
    </owl:NamedIndividual>
    


    <!-- http://purl.obolibrary.org/obo/GAZ_00141678 -->

    <owl:NamedIndividual rdf:about="http://purl.obolibrary.org/obo/GAZ_00141678">
        <obo:RO_0001025 rdf:resource="http://purl.obolibrary.org/obo/GAZ_00140392"/>
        <obo:IAO_0000115>A rocky island, 2.4 km long, lying 10 km northwest of Dint Island in Lazarev Bay, off the west side of Alexander Island.</obo:IAO_0000115>
        <oboInOwl:hasOBONamespace>GAZ</oboInOwl:hasOBONamespace>
        <oboInOwl:id>GAZ:00141678</oboInOwl:id>
        <rdfs:label>Umber Island</rdfs:label>
    </owl:NamedIndividual>
    


    <!-- http://purl.obolibrary.org/obo/GAZ_00141679 -->

    <owl:NamedIndividual rdf:about="http://purl.obolibrary.org/obo/GAZ_00141679">
        <obo:RO_0001025 rdf:resource="http://purl.obolibrary.org/obo/GAZ_00023294"/>
        <obo:IAO_0000115>An archipelago of three small islands lying 6 km west-northwest of Hamnenabben Head in the east part of Lutzow-Holm Bay.</obo:IAO_0000115>
        <oboInOwl:hasOBONamespace>GAZ</oboInOwl:hasOBONamespace>
        <oboInOwl:id>GAZ:00141679</oboInOwl:id>
        <rdfs:label>Ungane Islands</rdfs:label>
    </owl:NamedIndividual>
    


    <!-- http://purl.obolibrary.org/obo/GAZ_00141680 -->

    <owl:NamedIndividual rdf:about="http://purl.obolibrary.org/obo/GAZ_00141680">
        <obo:RO_0001025 rdf:resource="http://purl.obolibrary.org/obo/GAZ_00141554"/>
        <obo:IAO_0000115>An ice-covered island lying north of Halvfarryggen Ridge and between the Ekstrom and Jelbart Ice Shelves, on the coast of Queen Maud Land.</obo:IAO_0000115>
        <oboInOwl:hasOBONamespace>GAZ</oboInOwl:hasOBONamespace>
        <oboInOwl:id>GAZ:00141680</oboInOwl:id>
        <rdfs:label>Unneruskollen Island</rdfs:label>
    </owl:NamedIndividual>
    


    <!-- http://purl.obolibrary.org/obo/GAZ_00141681 -->

    <owl:NamedIndividual rdf:about="http://purl.obolibrary.org/obo/GAZ_00141681">
        <obo:RO_0001025 rdf:resource="http://purl.obolibrary.org/obo/GAZ_00141596"/>
        <obo:IAO_0000115>The largest and southernmost of the Bennett Islands, lying in Hanusse Bay.</obo:IAO_0000115>
        <oboInOwl:hasOBONamespace>GAZ</oboInOwl:hasOBONamespace>
        <oboInOwl:id>GAZ:00141681</oboInOwl:id>
        <rdfs:label>Weertman Island</rdfs:label>
    </owl:NamedIndividual>
    


    <!-- http://purl.obolibrary.org/obo/GAZ_00141682 -->

    <owl:NamedIndividual rdf:about="http://purl.obolibrary.org/obo/GAZ_00141682">
        <obo:RO_0001025 rdf:resource="http://purl.obolibrary.org/obo/GAZ_00045066"/>
        <obo:IAO_0000115>The western of two larger islands at the north end of the Flat Islands in Holme Bay, Mac Robertson Land.</obo:IAO_0000115>
        <oboInOwl:hasOBONamespace>GAZ</oboInOwl:hasOBONamespace>
        <oboInOwl:id>GAZ:00141682</oboInOwl:id>
        <rdfs:label>West Budd Island</rdfs:label>
    </owl:NamedIndividual>
    


    <!-- http://purl.obolibrary.org/obo/GAZ_00141683 -->

    <owl:NamedIndividual rdf:about="http://purl.obolibrary.org/obo/GAZ_00141683">
        <obo:RO_0001025 rdf:resource="http://purl.obolibrary.org/obo/GAZ_00023294"/>
        <obo:IAO_0000115>The largest of four islands in a cluster. It lies 6 km west of Langhovde Hills in the east part of Lutzow-Holm Bay.</obo:IAO_0000115>
        <oboInOwl:hasOBONamespace>GAZ</oboInOwl:hasOBONamespace>
        <oboInOwl:id>GAZ:00141683</oboInOwl:id>
        <rdfs:label>Ytrehovdeholmen</rdfs:label>
    </owl:NamedIndividual>
    


    <!-- http://purl.obolibrary.org/obo/GAZ_00141685 -->

    <owl:NamedIndividual rdf:about="http://purl.obolibrary.org/obo/GAZ_00141685">
        <rdf:type rdf:resource="http://purl.obolibrary.org/obo/ENVO_00000275"/>
        <obo:RO_0001025 rdf:resource="http://purl.obolibrary.org/obo/GAZ_00051499"/>
        <obo:IAO_0000115>An undersea trough.</obo:IAO_0000115>
        <oboInOwl:hasOBONamespace>GAZ</oboInOwl:hasOBONamespace>
        <oboInOwl:id>GAZ:00141685</oboInOwl:id>
        <rdfs:label>Lazarev Trough</rdfs:label>
    </owl:NamedIndividual>
    


    <!-- http://purl.obolibrary.org/obo/GAZ_00141686 -->

    <owl:NamedIndividual rdf:about="http://purl.obolibrary.org/obo/GAZ_00141686">
        <obo:RO_0001025 rdf:resource="http://purl.obolibrary.org/obo/GAZ_00004045"/>
        <obo:IAO_0000115>A natural harbour on the Antarctic Peninsula.</obo:IAO_0000115>
        <oboInOwl:hasOBONamespace>GAZ</oboInOwl:hasOBONamespace>
        <oboInOwl:id>GAZ:00141686</oboInOwl:id>
        <rdfs:label>Port Lockroy</rdfs:label>
    </owl:NamedIndividual>
    


    <!-- http://purl.obolibrary.org/obo/GAZ_00141687 -->

    <owl:NamedIndividual rdf:about="http://purl.obolibrary.org/obo/GAZ_00141687">
        <obo:RO_0001025 rdf:resource="http://purl.obolibrary.org/obo/GAZ_00141552"/>
        <obo:IAO_0000115>A channel in Antarctica. It is located between the southern end of Anvers and Wiencke Islands and the Wilhelm Archipelago.</obo:IAO_0000115>
        <oboInOwl:hasOBONamespace>GAZ</oboInOwl:hasOBONamespace>
        <oboInOwl:id>GAZ:00141687</oboInOwl:id>
        <rdfs:label>Bismarck Strait</rdfs:label>
    </owl:NamedIndividual>
    


    <!-- http://purl.obolibrary.org/obo/GAZ_00141688 -->

    <owl:NamedIndividual rdf:about="http://purl.obolibrary.org/obo/GAZ_00141688">
        <obo:RO_0001025 rdf:resource="http://purl.obolibrary.org/obo/GAZ_00140059"/>
        <obo:IAO_0000115>An island nearly 0.5 mi long, lying midway between Heywood Island and the W extremity of Robert Island, in the South Shetland Islands.</obo:IAO_0000115>
        <oboInOwl:hasOBONamespace>GAZ</oboInOwl:hasOBONamespace>
        <oboInOwl:id>GAZ:00141688</oboInOwl:id>
        <rdfs:label>Cornwall Island</rdfs:label>
    </owl:NamedIndividual>
    


    <!-- http://purl.obolibrary.org/obo/GAZ_00141689 -->

    <owl:NamedIndividual rdf:about="http://purl.obolibrary.org/obo/GAZ_00141689">
        <obo:RO_0001025 rdf:resource="http://purl.obolibrary.org/obo/GAZ_00140059"/>
        <obo:IAO_0000115>A 1.34 km wide cove indenting for 670 m the north coast of Robert Island, South Shetland Islands west of Lavrenov Point.</obo:IAO_0000115>
        <oboInOwl:hasOBONamespace>GAZ</oboInOwl:hasOBONamespace>
        <oboInOwl:id>GAZ:00141689</oboInOwl:id>
        <rdfs:label>Yundola Cove</rdfs:label>
    </owl:NamedIndividual>
    


    <!-- http://purl.obolibrary.org/obo/GAZ_00141690 -->

    <owl:NamedIndividual rdf:about="http://purl.obolibrary.org/obo/GAZ_00141690">
        <obo:RO_0001025 rdf:resource="http://purl.obolibrary.org/obo/GAZ_00007288"/>
        <obo:IAO_0000115>A peninsula extending 4 km in northeast-southwest direction and 2.8 km wide, forming the northwest extremity of Robert Island, South Shetland Islands. Bounded by Mitchell Cove, Carlota Cove, and Clothier Harbour. Linked to Coppermine Peninsula (1.7 km long and 500 m wide) in the west.</obo:IAO_0000115>
        <oboInOwl:hasOBONamespace>GAZ</oboInOwl:hasOBONamespace>
        <oboInOwl:id>GAZ:00141690</oboInOwl:id>
        <rdfs:label>Alfatar Peninsula</rdfs:label>
    </owl:NamedIndividual>
    


    <!-- http://purl.obolibrary.org/obo/GAZ_00141691 -->

    <owl:NamedIndividual rdf:about="http://purl.obolibrary.org/obo/GAZ_00141691">
        <rdf:type rdf:resource="http://purl.obolibrary.org/obo/ENVO_00000305"/>
        <obo:RO_0001025 rdf:resource="http://purl.obolibrary.org/obo/GAZ_00007288"/>
        <obo:IAO_0000115>A headland on the east coast of Robert Island, South Shetland Islands situated 1.2 km northwest of Perelik Point.</obo:IAO_0000115>
        <oboInOwl:hasOBONamespace>GAZ</oboInOwl:hasOBONamespace>
        <oboInOwl:id>GAZ:00141691</oboInOwl:id>
        <rdfs:label>Smirnenski Point</rdfs:label>
    </owl:NamedIndividual>
    


    <!-- http://purl.obolibrary.org/obo/GAZ_00141692 -->

    <owl:NamedIndividual rdf:about="http://purl.obolibrary.org/obo/GAZ_00141692">
        <obo:RO_0001025 rdf:resource="http://purl.obolibrary.org/obo/GAZ_00140059"/>
        <obo:IAO_0000115>A group of rocks off the northwest coast of Smith Island, South Shetland Islands. The two adjacent principal rocks extending 450 m in east-west direction and 100 m wide are situated 250 m north of Lista Point, with the third major one situated 400 m northwest of them.</obo:IAO_0000115>
        <oboInOwl:hasOBONamespace>GAZ</oboInOwl:hasOBONamespace>
        <oboInOwl:id>GAZ:00141692</oboInOwl:id>
        <rdfs:label>Maglizh Rocks</rdfs:label>
    </owl:NamedIndividual>
    


    <!-- http://purl.obolibrary.org/obo/GAZ_00141693 -->

    <owl:NamedIndividual rdf:about="http://purl.obolibrary.org/obo/GAZ_00141693">
        <obo:RO_0001025 rdf:resource="http://purl.obolibrary.org/obo/GAZ_00140059"/>
        <obo:IAO_0000115>A triangular island situated 120 m off the north coast of Robert Island, South Shetland Islands, and 950 m west-northwest of Newell Point.</obo:IAO_0000115>
        <oboInOwl:hasOBONamespace>GAZ</oboInOwl:hasOBONamespace>
        <oboInOwl:id>GAZ:00141693</oboInOwl:id>
        <rdfs:label>Tatul Island</rdfs:label>
    </owl:NamedIndividual>
    


    <!-- http://purl.obolibrary.org/obo/GAZ_00141694 -->

    <owl:NamedIndividual rdf:about="http://purl.obolibrary.org/obo/GAZ_00141694">
        <rdf:type rdf:resource="http://purl.obolibrary.org/obo/ENVO_00000305"/>
        <obo:RO_0001025 rdf:resource="http://purl.obolibrary.org/obo/GAZ_00007288"/>
        <obo:IAO_0000115>A headland on the east coast of Robert Island, South Shetland Islands situated 1.4 km northwest of Kitchen Point.</obo:IAO_0000115>
        <oboInOwl:hasOBONamespace>GAZ</oboInOwl:hasOBONamespace>
        <oboInOwl:id>GAZ:00141694</oboInOwl:id>
        <rdfs:label>Perelik Point</rdfs:label>
    </owl:NamedIndividual>
    


    <!-- http://purl.obolibrary.org/obo/GAZ_00141695 -->

    <owl:NamedIndividual rdf:about="http://purl.obolibrary.org/obo/GAZ_00141695">
        <obo:RO_0001025 rdf:resource="http://purl.obolibrary.org/obo/GAZ_00140059"/>
        <obo:IAO_0000115>The 700 m wide cove indenting for 400 m the northwest coast of Smith Island, South Shetland Islands west of Cape Smith.</obo:IAO_0000115>
        <oboInOwl:hasOBONamespace>GAZ</oboInOwl:hasOBONamespace>
        <oboInOwl:id>GAZ:00141695</oboInOwl:id>
        <rdfs:label>Glozhene Cove</rdfs:label>
    </owl:NamedIndividual>
    


    <!-- http://purl.obolibrary.org/obo/GAZ_00141696 -->

    <owl:NamedIndividual rdf:about="http://purl.obolibrary.org/obo/GAZ_00141696">
        <rdf:type rdf:resource="http://purl.obolibrary.org/obo/ENVO_00000305"/>
        <obo:RO_0001025 rdf:resource="http://purl.obolibrary.org/obo/GAZ_00007288"/>
        <obo:IAO_0000115>A headland on the north coast of Robert Island, South Shetland Islands situated 2.7 km west of Newell Point and 2.6 km southeast of Catharina Point.</obo:IAO_0000115>
        <oboInOwl:hasOBONamespace>GAZ</oboInOwl:hasOBONamespace>
        <oboInOwl:id>GAZ:00141696</oboInOwl:id>
        <rdfs:label>Lavrenov Point</rdfs:label>
    </owl:NamedIndividual>
    


    <!-- http://purl.obolibrary.org/obo/GAZ_00141697 -->

    <owl:NamedIndividual rdf:about="http://purl.obolibrary.org/obo/GAZ_00141697">
        <rdf:type rdf:resource="http://purl.obolibrary.org/obo/ENVO_00000305"/>
        <obo:RO_0001025 rdf:resource="http://purl.obolibrary.org/obo/GAZ_00007288"/>
        <obo:IAO_0000115>A headland on the northeast coast of Robert Island, South Shetland Islands situated 4.7 km west of Smirnenski Point, and 4.2 km southeast of Newell Point.</obo:IAO_0000115>
        <oboInOwl:hasOBONamespace>GAZ</oboInOwl:hasOBONamespace>
        <oboInOwl:id>GAZ:00141697</oboInOwl:id>
        <rdfs:label>Ugarchin Point</rdfs:label>
    </owl:NamedIndividual>
    


    <!-- http://purl.obolibrary.org/obo/GAZ_00141698 -->

    <owl:NamedIndividual rdf:about="http://purl.obolibrary.org/obo/GAZ_00141698">
        <rdf:type rdf:resource="http://purl.obolibrary.org/obo/ENVO_00000305"/>
        <obo:RO_0001025 rdf:resource="http://purl.obolibrary.org/obo/GAZ_00007288"/>
        <obo:IAO_0000115>A headland forming the northwest side of the entrance to Mitchell Cove in Robert Island, South Shetland Islands. Situated 2.75 km northwest of Negra Point and 4 km southeast of Fort William Point.</obo:IAO_0000115>
        <oboInOwl:hasOBONamespace>GAZ</oboInOwl:hasOBONamespace>
        <oboInOwl:id>GAZ:00141698</oboInOwl:id>
        <rdfs:label>Debelyanov Point</rdfs:label>
    </owl:NamedIndividual>
    


    <!-- http://purl.obolibrary.org/obo/GAZ_00141699 -->

    <owl:NamedIndividual rdf:about="http://purl.obolibrary.org/obo/GAZ_00141699">
        <obo:RO_0001025 rdf:resource="http://purl.obolibrary.org/obo/GAZ_00140059"/>
        <obo:IAO_0000115>A cove at the S extremity of Robert Island.</obo:IAO_0000115>
        <oboInOwl:hasOBONamespace>GAZ</oboInOwl:hasOBONamespace>
        <oboInOwl:id>GAZ:00141699</oboInOwl:id>
        <rdfs:label>Micalvi Cove</rdfs:label>
    </owl:NamedIndividual>
    


    <!-- http://purl.obolibrary.org/obo/GAZ_00141700 -->

    <owl:NamedIndividual rdf:about="http://purl.obolibrary.org/obo/GAZ_00141700">
        <obo:RO_0001025 rdf:resource="http://purl.obolibrary.org/obo/GAZ_00141699"/>
        <obo:IAO_0000115>Three adjacent rocks situated in the interior of Micalvi Cove in the south extremity of Robert Island, South Shetland Islands.</obo:IAO_0000115>
        <oboInOwl:hasOBONamespace>GAZ</oboInOwl:hasOBONamespace>
        <oboInOwl:id>GAZ:00141700</oboInOwl:id>
        <rdfs:label>Avren Rocks</rdfs:label>
    </owl:NamedIndividual>
    


    <!-- http://purl.obolibrary.org/obo/GAZ_00141701 -->

    <owl:NamedIndividual rdf:about="http://purl.obolibrary.org/obo/GAZ_00141701">
        <obo:RO_0001025 rdf:resource="http://purl.obolibrary.org/obo/GAZ_00140059"/>
        <obo:IAO_0000115>A 1.4 km wide cove indenting for 1.25 km the east coast of Robert Island, South Shetland Islands between Kitchen Point and Perelik Point.</obo:IAO_0000115>
        <oboInOwl:hasOBONamespace>GAZ</oboInOwl:hasOBONamespace>
        <oboInOwl:id>GAZ:00141701</oboInOwl:id>
        <rdfs:label>Kozloduy Cove</rdfs:label>
    </owl:NamedIndividual>
    


    <!-- http://purl.obolibrary.org/obo/GAZ_00141702 -->

    <owl:NamedIndividual rdf:about="http://purl.obolibrary.org/obo/GAZ_00141702">
        <obo:RO_0001025 rdf:resource="http://purl.obolibrary.org/obo/GAZ_00140059"/>
        <obo:IAO_0000115>An island off the northeast coast of Robert Island, South Shetland Islands situated 3.8 km northwest of Kitchen Point and 6.6 km southeast of Newell Point.</obo:IAO_0000115>
        <oboInOwl:hasOBONamespace>GAZ</oboInOwl:hasOBONamespace>
        <oboInOwl:id>GAZ:00141702</oboInOwl:id>
        <rdfs:label>Treklyano Island</rdfs:label>
    </owl:NamedIndividual>
    


    <!-- http://purl.obolibrary.org/obo/GAZ_00141703 -->

    <owl:NamedIndividual rdf:about="http://purl.obolibrary.org/obo/GAZ_00141703">
        <obo:RO_0001025 rdf:resource="http://purl.obolibrary.org/obo/GAZ_00140059"/>
        <obo:IAO_0000115>A group of rocks situated 1.8 km northeast of Treklyano Island off the northeast coast of Robert Island, South Shetland Islands.</obo:IAO_0000115>
        <oboInOwl:hasOBONamespace>GAZ</oboInOwl:hasOBONamespace>
        <oboInOwl:id>GAZ:00141703</oboInOwl:id>
        <rdfs:label>Makresh Rocks</rdfs:label>
    </owl:NamedIndividual>
    


    <!-- http://purl.obolibrary.org/obo/GAZ_00141704 -->

    <owl:NamedIndividual rdf:about="http://purl.obolibrary.org/obo/GAZ_00141704">
        <obo:RO_0001025 rdf:resource="http://purl.obolibrary.org/obo/GAZ_00140059"/>
        <obo:IAO_0000115>The 1.55 km wide cove indenting for 1.5 km the north coast of Robert Island, South Shetland Islands between Catharina Point and Hammer Point.</obo:IAO_0000115>
        <oboInOwl:hasOBONamespace>GAZ</oboInOwl:hasOBONamespace>
        <oboInOwl:id>GAZ:00141704</oboInOwl:id>
        <rdfs:label>Nevestino Cove</rdfs:label>
    </owl:NamedIndividual>
    


    <!-- http://purl.obolibrary.org/obo/GAZ_00141705 -->

    <owl:NamedIndividual rdf:about="http://purl.obolibrary.org/obo/GAZ_00141705">
        <obo:RO_0001025 rdf:resource="http://purl.obolibrary.org/obo/GAZ_00140059"/>
        <obo:IAO_0000115>Two adjacent islands situated 870 m east-northeast of Heywood Island and 2.1 km northwest of Catharina Point on Robert Island, South Shetland Islands.</obo:IAO_0000115>
        <oboInOwl:hasOBONamespace>GAZ</oboInOwl:hasOBONamespace>
        <oboInOwl:id>GAZ:00141705</oboInOwl:id>
        <rdfs:label>Pordim Islands</rdfs:label>
    </owl:NamedIndividual>
    


    <!-- http://purl.obolibrary.org/obo/GAZ_00141706 -->

    <owl:NamedIndividual rdf:about="http://purl.obolibrary.org/obo/GAZ_00141706">
        <obo:RO_0001025 rdf:resource="http://purl.obolibrary.org/obo/GAZ_00140059"/>
        <obo:IAO_0000115>A group of rocks with the principal one situated 700 m north of Henfield Rock and 3.44 km east of Pordim Islands off the north coast of Robert Island, South Shetland Islands.</obo:IAO_0000115>
        <oboInOwl:hasOBONamespace>GAZ</oboInOwl:hasOBONamespace>
        <oboInOwl:id>GAZ:00141706</oboInOwl:id>
        <rdfs:label>Opaka Rocks</rdfs:label>
    </owl:NamedIndividual>
    


    <!-- http://purl.obolibrary.org/obo/GAZ_00141707 -->

    <owl:NamedIndividual rdf:about="http://purl.obolibrary.org/obo/GAZ_00141707">
        <obo:RO_0001025 rdf:resource="http://purl.obolibrary.org/obo/GAZ_00140059"/>
        <obo:IAO_0000115>A rocky, crescent-shaped island lying 1.5 mi WNW of the N tip of Robert Island, in the South Shetland Islands.</obo:IAO_0000115>
        <oboInOwl:hasOBONamespace>GAZ</oboInOwl:hasOBONamespace>
        <oboInOwl:id>GAZ:00141707</oboInOwl:id>
        <rdfs:label>Heywood Island</rdfs:label>
    </owl:NamedIndividual>
    


    <!-- http://purl.obolibrary.org/obo/GAZ_00141708 -->

    <owl:NamedIndividual rdf:about="http://purl.obolibrary.org/obo/GAZ_00141708">
        <obo:RO_0001025 rdf:resource="http://purl.obolibrary.org/obo/GAZ_00140059"/>
        <obo:IAO_0000115>A conspicuous island off the north coast of Robert Island, South Shetland Islands situated 470 m south-southwest of Heywood Island and 920 m north-northeast of Cornwall Island.</obo:IAO_0000115>
        <oboInOwl:hasOBONamespace>GAZ</oboInOwl:hasOBONamespace>
        <oboInOwl:id>GAZ:00141708</oboInOwl:id>
        <rdfs:label>Rogozen Island</rdfs:label>
    </owl:NamedIndividual>
    


    <!-- http://purl.obolibrary.org/obo/GAZ_00141772 -->

    <owl:NamedIndividual rdf:about="http://purl.obolibrary.org/obo/GAZ_00141772">
        <obo:RO_0001025 rdf:resource="http://purl.obolibrary.org/obo/GAZ_00004045"/>
        <obo:IAO_0000115>A group of rocks off the northwest coast of Trinity Peninsula, Antarctica in the approach to Huon Bay, 4.8 km northeast of Cape Ducorps.</obo:IAO_0000115>
        <oboInOwl:hasOBONamespace>GAZ</oboInOwl:hasOBONamespace>
        <oboInOwl:id>GAZ:00141772</oboInOwl:id>
        <rdfs:label>De Mas Rocks</rdfs:label>
    </owl:NamedIndividual>
    


    <!-- http://purl.obolibrary.org/obo/GAZ_00141773 -->

    <owl:NamedIndividual rdf:about="http://purl.obolibrary.org/obo/GAZ_00141773">
        <obo:RO_0001025 rdf:resource="http://purl.obolibrary.org/obo/GAZ_00140668"/>
        <obo:IAO_0000115>A Bulgarian Antarctic base on Livingston Island in the South Shetland Islands. Located at an elevation of 12 to 15 m on Bulgarian Beach, 130 m inland from the shore of Emona Anchorage, east-northeast of Hesperides Point and southwest by west of Sinemorets Hill, overlooking the Grand Lagoon.</obo:IAO_0000115>
        <oboInOwl:hasOBONamespace>GAZ</oboInOwl:hasOBONamespace>
        <oboInOwl:id>GAZ:00141773</oboInOwl:id>
        <rdfs:label>St. Kliment Ohridski Base</rdfs:label>
    </owl:NamedIndividual>
    


    <!-- http://purl.obolibrary.org/obo/GAZ_00141774 -->

    <owl:NamedIndividual rdf:about="http://purl.obolibrary.org/obo/GAZ_00141774">
        <obo:RO_0001025 rdf:resource="http://purl.obolibrary.org/obo/GAZ_00017736"/>
        <obo:IAO_0000115>An inactive seasonal station operated by Argentina opened in 1953.</obo:IAO_0000115>
        <oboInOwl:hasOBONamespace>GAZ</oboInOwl:hasOBONamespace>
        <oboInOwl:id>GAZ:00141774</oboInOwl:id>
        <rdfs:label>Camara Base</rdfs:label>
    </owl:NamedIndividual>
    


    <!-- http://purl.obolibrary.org/obo/GAZ_00141775 -->

    <owl:NamedIndividual rdf:about="http://purl.obolibrary.org/obo/GAZ_00141775">
        <rdf:type rdf:resource="http://purl.obolibrary.org/obo/ENVO_00000305"/>
        <obo:RO_0001025 rdf:resource="http://purl.obolibrary.org/obo/GAZ_00007329"/>
        <obo:IAO_0000115>A headland forming the southwest extremity of Livingston Island, in the South Shetland Islands.</obo:IAO_0000115>
        <oboInOwl:hasOBONamespace>GAZ</oboInOwl:hasOBONamespace>
        <oboInOwl:id>GAZ:00141775</oboInOwl:id>
        <rdfs:label>Devils Point</rdfs:label>
    </owl:NamedIndividual>
    


    <!-- http://purl.obolibrary.org/obo/GAZ_00141776 -->

    <owl:NamedIndividual rdf:about="http://purl.obolibrary.org/obo/GAZ_00141776">
        <obo:RO_0001025 rdf:resource="http://purl.obolibrary.org/obo/GAZ_00007330"/>
        <obo:IAO_0000115>A Spanish seasonal encampment situated 1.2 km north of Nikopol Point on Byers Peninsula, Livingston Island, in the South Shetland Islands.</obo:IAO_0000115>
        <oboInOwl:hasOBONamespace>GAZ</oboInOwl:hasOBONamespace>
        <oboInOwl:id>GAZ:00141776</oboInOwl:id>
        <rdfs:label>Camp Byers</rdfs:label>
    </owl:NamedIndividual>
    


    <!-- http://purl.obolibrary.org/obo/GAZ_00141777 -->

    <owl:NamedIndividual rdf:about="http://purl.obolibrary.org/obo/GAZ_00141777">
        <rdf:type rdf:resource="http://purl.obolibrary.org/obo/ENVO_00000305"/>
        <obo:RO_0001025 rdf:resource="http://purl.obolibrary.org/obo/GAZ_00007329"/>
        <obo:IAO_0000115>A headland located on the south coast of Livingston Island, projecting 600 m into Bransfield Strait.</obo:IAO_0000115>
        <oboInOwl:hasOBONamespace>GAZ</oboInOwl:hasOBONamespace>
        <oboInOwl:id>GAZ:00141777</oboInOwl:id>
        <rdfs:label>Nikopol Point</rdfs:label>
    </owl:NamedIndividual>
    


    <!-- http://purl.obolibrary.org/obo/GAZ_00141778 -->

    <owl:NamedIndividual rdf:about="http://purl.obolibrary.org/obo/GAZ_00141778">
        <obo:RO_0001025 rdf:resource="http://purl.obolibrary.org/obo/GAZ_00007329"/>
        <obo:IAO_0000115>A series of elevations extending southwest from Leslie Hill in the eastern part of Livingston Island, in the South Shetland Islands.</obo:IAO_0000115>
        <oboInOwl:hasOBONamespace>GAZ</oboInOwl:hasOBONamespace>
        <oboInOwl:id>GAZ:00141778</oboInOwl:id>
        <rdfs:label>Gleaner Heights</rdfs:label>
    </owl:NamedIndividual>
    


    <!-- http://purl.obolibrary.org/obo/GAZ_00141779 -->

    <owl:NamedIndividual rdf:about="http://purl.obolibrary.org/obo/GAZ_00141779">
        <obo:RO_0001025 rdf:resource="http://purl.obolibrary.org/obo/GAZ_00007329"/>
        <obo:IAO_0000115>A small beach lying 1 mi southeast of Scarborough Castle on the north coast of Livingston Island, in the South Shetland Islands.</obo:IAO_0000115>
        <oboInOwl:hasOBONamespace>GAZ</oboInOwl:hasOBONamespace>
        <oboInOwl:id>GAZ:00141779</oboInOwl:id>
        <rdfs:label>Half Moon Beach</rdfs:label>
    </owl:NamedIndividual>
    


    <!-- http://purl.obolibrary.org/obo/GAZ_00141780 -->

    <owl:NamedIndividual rdf:about="http://purl.obolibrary.org/obo/GAZ_00141780">
        <obo:RO_0001025 rdf:resource="http://purl.obolibrary.org/obo/GAZ_00140059"/>
        <obo:IAO_0000115>A narrow boat passage between the rocks off Devils Point, the southwest end of Livingston Island, in the South Shetland Islands.</obo:IAO_0000115>
        <oboInOwl:hasOBONamespace>GAZ</oboInOwl:hasOBONamespace>
        <oboInOwl:id>GAZ:00141780</oboInOwl:id>
        <rdfs:label>Hell Gates</rdfs:label>
    </owl:NamedIndividual>
    


    <!-- http://purl.obolibrary.org/obo/GAZ_00141781 -->

    <owl:NamedIndividual rdf:about="http://purl.obolibrary.org/obo/GAZ_00141781">
        <rdf:type rdf:resource="http://purl.obolibrary.org/obo/ENVO_00000305"/>
        <obo:RO_0001025 rdf:resource="http://purl.obolibrary.org/obo/GAZ_00007329"/>
        <obo:IAO_0000115>A headland of land projecting into South Bay 1.4 km north of Johnsons Dock, Livingston Island in the South Shetland Islands, Antarctica.</obo:IAO_0000115>
        <oboInOwl:hasOBONamespace>GAZ</oboInOwl:hasOBONamespace>
        <oboInOwl:id>GAZ:00141781</oboInOwl:id>
        <rdfs:label>Hesperides Point</rdfs:label>
    </owl:NamedIndividual>
    


    <!-- http://purl.obolibrary.org/obo/GAZ_00141782 -->

    <owl:NamedIndividual rdf:about="http://purl.obolibrary.org/obo/GAZ_00141782">
        <obo:RO_0001025 rdf:resource="http://purl.obolibrary.org/obo/GAZ_00007329"/>
        <obo:IAO_0000115>The land between South Bay and False Bay on the south coast of Livingston Island, in the South Shetland Islands.</obo:IAO_0000115>
        <oboInOwl:hasOBONamespace>GAZ</oboInOwl:hasOBONamespace>
        <oboInOwl:id>GAZ:00141782</oboInOwl:id>
        <rdfs:label>Hurd Peninsula</rdfs:label>
    </owl:NamedIndividual>
    


    <!-- http://purl.obolibrary.org/obo/GAZ_00141783 -->

    <owl:NamedIndividual rdf:about="http://purl.obolibrary.org/obo/GAZ_00141783">
        <obo:RO_0001025 rdf:resource="http://purl.obolibrary.org/obo/GAZ_00007329"/>
        <obo:IAO_0000115>A beach at the west side of the entrance to Walker Bay on the south coast of Livingston Island, in the South Shetland Islands.</obo:IAO_0000115>
        <oboInOwl:hasOBONamespace>GAZ</oboInOwl:hasOBONamespace>
        <oboInOwl:id>GAZ:00141783</oboInOwl:id>
        <rdfs:label>John Beach</rdfs:label>
    </owl:NamedIndividual>
    


    <!-- http://purl.obolibrary.org/obo/GAZ_00141784 -->

    <owl:NamedIndividual rdf:about="http://purl.obolibrary.org/obo/GAZ_00141784">
        <obo:RO_0001025 rdf:resource="http://purl.obolibrary.org/obo/GAZ_00141782"/>
        <obo:IAO_0000115>A seasonal station operated by Spain opened in 1988. Situated on the South Bay of Hurd Peninsula on Livingston Island in the South Shetland Islands.</obo:IAO_0000115>
        <oboInOwl:hasOBONamespace>GAZ</oboInOwl:hasOBONamespace>
        <oboInOwl:id>GAZ:00141784</oboInOwl:id>
        <rdfs:label>Juan Carlos I Base</rdfs:label>
    </owl:NamedIndividual>
    


    <!-- http://purl.obolibrary.org/obo/GAZ_00141785 -->

    <owl:NamedIndividual rdf:about="http://purl.obolibrary.org/obo/GAZ_00141785">
        <obo:RO_0001025 rdf:resource="http://purl.obolibrary.org/obo/GAZ_00140059"/>
        <obo:IAO_0000115>The strait between Snow Island on the southwest and Rugged and Livingston Islands on the northeast, in the South Shetland Islands.</obo:IAO_0000115>
        <oboInOwl:hasOBONamespace>GAZ</oboInOwl:hasOBONamespace>
        <oboInOwl:id>GAZ:00141785</oboInOwl:id>
        <rdfs:label>Morton Strait</rdfs:label>
    </owl:NamedIndividual>
    


    <!-- http://purl.obolibrary.org/obo/GAZ_00141786 -->

    <owl:NamedIndividual rdf:about="http://purl.obolibrary.org/obo/GAZ_00141786">
        <rdf:type rdf:resource="http://purl.obolibrary.org/obo/ENVO_00000167"/>
        <obo:RO_0001025 rdf:resource="http://purl.obolibrary.org/obo/GAZ_00007329"/>
        <obo:IAO_0000115>A narrow point forming the east extremity of Livingston Island, in the South Shetland Islands.</obo:IAO_0000115>
        <oboInOwl:hasOBONamespace>GAZ</oboInOwl:hasOBONamespace>
        <oboInOwl:id>GAZ:00141786</oboInOwl:id>
        <rdfs:label>Renier Point</rdfs:label>
    </owl:NamedIndividual>
    


    <!-- http://purl.obolibrary.org/obo/GAZ_00141787 -->

    <owl:NamedIndividual rdf:about="http://purl.obolibrary.org/obo/GAZ_00141787">
        <obo:RO_0001025 rdf:resource="http://purl.obolibrary.org/obo/GAZ_00007330"/>
        <obo:IAO_0000115>Beaches extending along the north side of Byers Peninsula, Livingston Island in the South Shetland Islands.</obo:IAO_0000115>
        <oboInOwl:hasOBONamespace>GAZ</oboInOwl:hasOBONamespace>
        <oboInOwl:id>GAZ:00141787</oboInOwl:id>
        <rdfs:label>Robbery Beaches</rdfs:label>
    </owl:NamedIndividual>
    


    <!-- http://purl.obolibrary.org/obo/GAZ_00141788 -->

    <owl:NamedIndividual rdf:about="http://purl.obolibrary.org/obo/GAZ_00141788">
        <obo:RO_0001025 rdf:resource="http://purl.obolibrary.org/obo/GAZ_00007328"/>
        <obo:IAO_0000115>An island forming the west side of Shirreff Cove on the north coast of Livingston Island, in the South Shetland Islands.</obo:IAO_0000115>
        <oboInOwl:hasOBONamespace>GAZ</oboInOwl:hasOBONamespace>
        <oboInOwl:id>GAZ:00141788</oboInOwl:id>
        <rdfs:label>San Telmo Island</rdfs:label>
    </owl:NamedIndividual>
    


    <!-- http://purl.obolibrary.org/obo/GAZ_00141789 -->

    <owl:NamedIndividual rdf:about="http://purl.obolibrary.org/obo/GAZ_00141789">
        <obo:RO_0001025 rdf:resource="http://purl.obolibrary.org/obo/GAZ_00140059"/>
        <obo:IAO_0000115>A small cove or anchorage, situated immediately southwest of Cape Shirreff along the north side of Livingston Island, in the South Shetland Islands.</obo:IAO_0000115>
        <oboInOwl:hasOBONamespace>GAZ</oboInOwl:hasOBONamespace>
        <oboInOwl:id>GAZ:00141789</oboInOwl:id>
        <rdfs:label>Shirreff Cove</rdfs:label>
    </owl:NamedIndividual>
    


    <!-- http://purl.obolibrary.org/obo/GAZ_00141790 -->

    <owl:NamedIndividual rdf:about="http://purl.obolibrary.org/obo/GAZ_00141790">
        <obo:RO_0001025 rdf:resource="http://purl.obolibrary.org/obo/GAZ_00139751"/>
        <obo:IAO_0000115>A seasonal field station operated by Chile and the USA opened in 1991. Situated on the east side of Cape Shirreff on Ioannes Paulus II Peninsula on Livingston Island in the South Shetland Islands.</obo:IAO_0000115>
        <oboInOwl:hasOBONamespace>GAZ</oboInOwl:hasOBONamespace>
        <oboInOwl:id>GAZ:00141790</oboInOwl:id>
        <rdfs:label>Shirreff Base</rdfs:label>
    </owl:NamedIndividual>
    


    <!-- http://purl.obolibrary.org/obo/GAZ_00141791 -->

    <owl:NamedIndividual rdf:about="http://purl.obolibrary.org/obo/GAZ_00141791">
        <rdf:type rdf:resource="http://purl.obolibrary.org/obo/ENVO_00000305"/>
        <obo:RO_0001025 rdf:resource="http://purl.obolibrary.org/obo/GAZ_00007329"/>
        <obo:IAO_0000115>A headland marking the northwest end of Livingston Island, in the South Shetland Islands.</obo:IAO_0000115>
        <oboInOwl:hasOBONamespace>GAZ</oboInOwl:hasOBONamespace>
        <oboInOwl:id>GAZ:00141791</oboInOwl:id>
        <rdfs:label>Start Point</rdfs:label>
    </owl:NamedIndividual>
    


    <!-- http://purl.obolibrary.org/obo/GAZ_00141792 -->

    <owl:NamedIndividual rdf:about="http://purl.obolibrary.org/obo/GAZ_00141792">
        <rdf:type rdf:resource="http://purl.obolibrary.org/obo/ENVO_00000305"/>
        <obo:RO_0001025 rdf:resource="http://purl.obolibrary.org/obo/GAZ_00017735"/>
        <obo:IAO_0000115>A headland forming the west extremity of Greenwich Island, in the South Shetland Islands, Antarctica.</obo:IAO_0000115>
        <oboInOwl:hasOBONamespace>GAZ</oboInOwl:hasOBONamespace>
        <oboInOwl:id>GAZ:00141792</oboInOwl:id>
        <rdfs:label>Duff Point</rdfs:label>
    </owl:NamedIndividual>
    


    <!-- http://purl.obolibrary.org/obo/GAZ_00141793 -->

    <owl:NamedIndividual rdf:about="http://purl.obolibrary.org/obo/GAZ_00141793">
        <obo:RO_0001025 rdf:resource="http://purl.obolibrary.org/obo/GAZ_00007288"/>
        <obo:IAO_0000115>An ice-free point on the southwest coast of Robert Island situated 6.8 km southeast of Negra Point, 1.8 km east-southeast of Beron Point, and 2 km northwest of Edwards Point. Forming the northwest side of the entrance to Micalvi Cove.</obo:IAO_0000115>
        <oboInOwl:hasOBONamespace>GAZ</oboInOwl:hasOBONamespace>
        <oboInOwl:id>GAZ:00141793</oboInOwl:id>
        <rdfs:label>Zahari Point</rdfs:label>
    </owl:NamedIndividual>
    


    <!-- http://purl.obolibrary.org/obo/GAZ_00141794 -->

    <owl:NamedIndividual rdf:about="http://purl.obolibrary.org/obo/GAZ_00141794">
        <rdf:type rdf:resource="http://purl.obolibrary.org/obo/ENVO_00000305"/>
        <obo:RO_0001025 rdf:resource="http://purl.obolibrary.org/obo/GAZ_00017735"/>
        <obo:IAO_0000115>A headland on the southwest coast of Greenwich Island, Antarctica situated next west of Hebrizelm Hill, 1.3 km west-northwest of Triangle Point, 2 km south-southwest of Tile Ridge, and 2 km southeast of Yovkov Point.</obo:IAO_0000115>
        <oboInOwl:hasOBONamespace>GAZ</oboInOwl:hasOBONamespace>
        <oboInOwl:id>GAZ:00141794</oboInOwl:id>
        <rdfs:label>Kaspichan Point</rdfs:label>
    </owl:NamedIndividual>
    


    <!-- http://purl.obolibrary.org/obo/GAZ_00141795 -->

    <owl:NamedIndividual rdf:about="http://purl.obolibrary.org/obo/GAZ_00141795">
        <rdf:type rdf:resource="http://purl.obolibrary.org/obo/ENVO_00000305"/>
        <obo:RO_0001025 rdf:resource="http://purl.obolibrary.org/obo/GAZ_00017735"/>
        <obo:IAO_0000115>A headland on the southwest coast of Greenwich Island, Antarctica situated 3.6 km southeast of Kerseblept Nunatak, 2.2 km south-southwest of Lloyd Hill, 2.8 km southwest of Tile Ridge, and 2.1 km west-northwest of Hebrizelm Hill.</obo:IAO_0000115>
        <oboInOwl:hasOBONamespace>GAZ</oboInOwl:hasOBONamespace>
        <oboInOwl:id>GAZ:00141795</oboInOwl:id>
        <rdfs:label>Yovkov Point</rdfs:label>
    </owl:NamedIndividual>
    


    <!-- http://purl.obolibrary.org/obo/GAZ_00141796 -->

    <owl:NamedIndividual rdf:about="http://purl.obolibrary.org/obo/GAZ_00141796">
        <rdf:type rdf:resource="http://purl.obolibrary.org/obo/ENVO_00000305"/>
        <obo:RO_0001025 rdf:resource="http://purl.obolibrary.org/obo/GAZ_00017735"/>
        <obo:IAO_0000115>A headland that projects 600 m from the north coast of Greenwich Island in the South Shetland Islands, Antarctica and is snow-free in summer.</obo:IAO_0000115>
        <oboInOwl:hasOBONamespace>GAZ</oboInOwl:hasOBONamespace>
        <oboInOwl:id>GAZ:00141796</oboInOwl:id>
        <rdfs:label>Pavlikeni Point</rdfs:label>
    </owl:NamedIndividual>
    


    <!-- http://purl.obolibrary.org/obo/GAZ_00141797 -->

    <owl:NamedIndividual rdf:about="http://purl.obolibrary.org/obo/GAZ_00141797">
        <obo:RO_0001025 rdf:resource="http://purl.obolibrary.org/obo/GAZ_00129076"/>
        <obo:IAO_0000115>A headland forming both the south extremity and the vertex of the V-shaped Desolation Island situated in the entrance to Hero Bay, Livingston Island, Antarctica. Separated from Miladinovi Islets to the south by Neck or Nothing Passage.</obo:IAO_0000115>
        <oboInOwl:hasOBONamespace>GAZ</oboInOwl:hasOBONamespace>
        <oboInOwl:id>GAZ:00141797</oboInOwl:id>
        <rdfs:label>Iratais Point</rdfs:label>
    </owl:NamedIndividual>
    


    <!-- http://purl.obolibrary.org/obo/GAZ_00141804 -->

    <owl:NamedIndividual rdf:about="http://purl.obolibrary.org/obo/GAZ_00141804">
        <obo:RO_0001025 rdf:resource="http://purl.obolibrary.org/obo/GAZ_00005837"/>
        <obo:IAO_0000115>The highest point (1,755 meters) in Peter I Island, off the coast of Antarctica. A shield volcano.</obo:IAO_0000115>
        <oboInOwl:hasOBONamespace>GAZ</oboInOwl:hasOBONamespace>
        <oboInOwl:id>GAZ:00141804</oboInOwl:id>
        <rdfs:label>Lars Christensen Peak</rdfs:label>
    </owl:NamedIndividual>
    


    <!-- http://purl.obolibrary.org/obo/GAZ_00141869 -->

    <owl:NamedIndividual rdf:about="http://purl.obolibrary.org/obo/GAZ_00141869">
        <obo:RO_0001025 rdf:resource="http://purl.obolibrary.org/obo/GAZ_00004380"/>
        <obo:IAO_0000115>An island located off the coast of the Antarctic Peninsula. It is once thought to be part of a larger island known as Anvers Island because the gap between the islands was covered by the Marr Ice Piedmont. Rapid recession of the ice revealed this as a separate island in 2004.</obo:IAO_0000115>
        <oboInOwl:hasOBONamespace>GAZ</oboInOwl:hasOBONamespace>
        <oboInOwl:id>GAZ:00141869</oboInOwl:id>
        <rdfs:label>Amsler Island</rdfs:label>
    </owl:NamedIndividual>
    


    <!-- http://purl.obolibrary.org/obo/GAZ_00141870 -->

    <owl:NamedIndividual rdf:about="http://purl.obolibrary.org/obo/GAZ_00141870">
        <obo:RO_0001025 rdf:resource="http://purl.obolibrary.org/obo/GAZ_00141480"/>
        <obo:IAO_0000115>A circular island 1.6 km in diameter, consisting of a high plateau with steep slopes surmounted on the northwest side by a pyramidal peak 450 m high, lying in the northeast entrance to Admiralty Sound, south of the northeast end of Antarctic Peninsula.</obo:IAO_0000115>
        <oboInOwl:hasOBONamespace>GAZ</oboInOwl:hasOBONamespace>
        <oboInOwl:id>GAZ:00141870</oboInOwl:id>
        <rdfs:label>Cockburn Island</rdfs:label>
    </owl:NamedIndividual>
    


    <!-- http://purl.obolibrary.org/obo/GAZ_00141871 -->

    <owl:NamedIndividual rdf:about="http://purl.obolibrary.org/obo/GAZ_00141871">
        <obo:RO_0001025 rdf:resource="http://purl.obolibrary.org/obo/GAZ_00004045"/>
        <obo:IAO_0000115>An sland nearly 1 mile long, lying 1.5 miles southeast of Bonaparte Point, off the southwest coast of Anvers Island in the Palmer Archipelago.</obo:IAO_0000115>
        <oboInOwl:hasOBONamespace>GAZ</oboInOwl:hasOBONamespace>
        <oboInOwl:id>GAZ:00141871</oboInOwl:id>
        <rdfs:label>Hermit Island</rdfs:label>
    </owl:NamedIndividual>
    


    <!-- http://purl.obolibrary.org/obo/GAZ_00141907 -->

    <owl:NamedIndividual rdf:about="http://purl.obolibrary.org/obo/GAZ_00141907">
        <obo:RO_0001025 rdf:resource="http://purl.obolibrary.org/obo/GAZ_00007425"/>
        <obo:IAO_0000115>A Polish research station on King George Island, off the coast of Antarctica. Established 1977-02-26.</obo:IAO_0000115>
        <oboInOwl:hasOBONamespace>GAZ</oboInOwl:hasOBONamespace>
        <oboInOwl:id>GAZ:00141907</oboInOwl:id>
        <rdfs:label>Henryk Arctowski Polish Antarctic Station</rdfs:label>
    </owl:NamedIndividual>
    


    <!-- http://purl.obolibrary.org/obo/GAZ_00141908 -->

    <owl:NamedIndividual rdf:about="http://purl.obolibrary.org/obo/GAZ_00141908">
        <obo:RO_0001025 rdf:resource="http://purl.obolibrary.org/obo/GAZ_00007425"/>
        <obo:IAO_0000115>An Argentine permanent base in King George Island. Established 1982.</obo:IAO_0000115>
        <oboInOwl:hasOBONamespace>GAZ</oboInOwl:hasOBONamespace>
        <oboInOwl:id>GAZ:00141908</oboInOwl:id>
        <rdfs:label>Jubany</rdfs:label>
    </owl:NamedIndividual>
    


    <!-- http://purl.obolibrary.org/obo/GAZ_00141909 -->

    <owl:NamedIndividual rdf:about="http://purl.obolibrary.org/obo/GAZ_00141909">
        <obo:RO_0001025 rdf:resource="http://purl.obolibrary.org/obo/GAZ_00023302"/>
        <obo:IAO_0000115>A British research station. Established 1975.</obo:IAO_0000115>
        <oboInOwl:hasOBONamespace>GAZ</oboInOwl:hasOBONamespace>
        <oboInOwl:id>GAZ:00141909</oboInOwl:id>
        <rdfs:label>Rothera Research Station</rdfs:label>
    </owl:NamedIndividual>
    


    <!-- http://purl.obolibrary.org/obo/GAZ_00141910 -->

    <owl:NamedIndividual rdf:about="http://purl.obolibrary.org/obo/GAZ_00141910">
        <obo:RO_0001025 rdf:resource="http://purl.obolibrary.org/obo/GAZ_00007425"/>
        <obo:IAO_0000115>A Peruvian research station on the coast of Admiralty Bay. Established 1989.</obo:IAO_0000115>
        <oboInOwl:hasOBONamespace>GAZ</oboInOwl:hasOBONamespace>
        <oboInOwl:id>GAZ:00141910</oboInOwl:id>
        <rdfs:label>Machu Picchu Scientific Base</rdfs:label>
    </owl:NamedIndividual>
    


    <!-- http://purl.obolibrary.org/obo/GAZ_00141918 -->

    <owl:NamedIndividual rdf:about="http://purl.obolibrary.org/obo/GAZ_00141918">
        <obo:RO_0001025 rdf:resource="http://purl.obolibrary.org/obo/GAZ_00045077"/>
        <obo:IAO_0000115>A Czech research station built in Antarctica, on the coast of James Ross Island. Established 2006.</obo:IAO_0000115>
        <oboInOwl:hasOBONamespace>GAZ</oboInOwl:hasOBONamespace>
        <oboInOwl:id>GAZ:00141918</oboInOwl:id>
        <rdfs:label>Johann Gregor Mendel Czech Antarctic Station</rdfs:label>
    </owl:NamedIndividual>
    


    <!-- http://purl.obolibrary.org/obo/GAZ_00143780 -->

    <owl:NamedIndividual rdf:about="http://purl.obolibrary.org/obo/GAZ_00143780">
        <obo:RO_0001025 rdf:resource="http://purl.obolibrary.org/obo/GAZ_00000373"/>
        <obo:IAO_0000115>One of three major basins in the Southern Ocean. It extends from its western border with the Pacific-Antarctic Basin at the Scotia Ridge and Drake Passage (at about 70degW) to its eastern border with the Australian-Atlantic Basin at the Kerguelan Plateau (about 75degE). It consists of the Enderby and Weddell Abyssal Plains and is bounded to the north below 4000 m by the Mid-Atlantic and South-West Indian Ridges except for deeper connections into the Argentine Basin in the western Atlantic and into the deep basins of the western Indian Ocean.</obo:IAO_0000115>
        <oboInOwl:hasOBONamespace>GAZ</oboInOwl:hasOBONamespace>
        <oboInOwl:id>GAZ:00143780</oboInOwl:id>
        <rdfs:label>Atlantic-Indian Basin</rdfs:label>
    </owl:NamedIndividual>
    


    <!-- http://purl.obolibrary.org/obo/GAZ_00143781 -->

    <owl:NamedIndividual rdf:about="http://purl.obolibrary.org/obo/GAZ_00143781">
        <obo:RO_0001025 rdf:resource="http://purl.obolibrary.org/obo/GAZ_00143780"/>
        <oboInOwl:hasOBONamespace>GAZ</oboInOwl:hasOBONamespace>
        <oboInOwl:id>GAZ:00143781</oboInOwl:id>
        <rdfs:label>Weddell Abyssal Plain</rdfs:label>
    </owl:NamedIndividual>
    


    <!-- http://purl.obolibrary.org/obo/GAZ_00143782 -->

    <owl:NamedIndividual rdf:about="http://purl.obolibrary.org/obo/GAZ_00143782">
        <obo:RO_0001025 rdf:resource="http://purl.obolibrary.org/obo/GAZ_00143780"/>
        <oboInOwl:hasOBONamespace>GAZ</oboInOwl:hasOBONamespace>
        <oboInOwl:id>GAZ:00143782</oboInOwl:id>
        <rdfs:label>Enderby Abyssal Plain</rdfs:label>
    </owl:NamedIndividual>
    


    <!-- http://purl.obolibrary.org/obo/GAZ_00143783 -->

    <owl:NamedIndividual rdf:about="http://purl.obolibrary.org/obo/GAZ_00143783">
        <obo:RO_0001025 rdf:resource="http://purl.obolibrary.org/obo/GAZ_00000373"/>
        <obo:IAO_0000115>One of three major basins in the Southern Ocean. It extends from its western border with the Australian-Antarctic Basin at the longitude of Tasmania (about 145degE) to its eastern border with the Atlantic-Indian Basin at the Scotia Ridge and Drake Passage (about 70degW). It consists of the Amundsen, Bellingshausen, and Mornington Abyssal Plains and is separated from the basins further north in the Pacific by the Pacific-Antarctic Ridge and the East Pacific Rise in the east and by the Chile rise in the east.</obo:IAO_0000115>
        <oboInOwl:hasOBONamespace>GAZ</oboInOwl:hasOBONamespace>
        <oboInOwl:id>GAZ:00143783</oboInOwl:id>
        <rdfs:label>Pacific-Antarctic Basin</rdfs:label>
    </owl:NamedIndividual>
    


    <!-- http://purl.obolibrary.org/obo/GAZ_00143784 -->

    <owl:NamedIndividual rdf:about="http://purl.obolibrary.org/obo/GAZ_00143784">
        <obo:RO_0001025 rdf:resource="http://purl.obolibrary.org/obo/GAZ_00143783"/>
        <obo:IAO_0000115>One of three plains that comprise the Pacific-Antarctic Basin. It is located at around 85-95degW.</obo:IAO_0000115>
        <oboInOwl:hasOBONamespace>GAZ</oboInOwl:hasOBONamespace>
        <oboInOwl:id>GAZ:00143784</oboInOwl:id>
        <rdfs:label>Mornington Abyssal Plain</rdfs:label>
    </owl:NamedIndividual>
    


    <!-- http://purl.obolibrary.org/obo/GAZ_00143785 -->

    <owl:NamedIndividual rdf:about="http://purl.obolibrary.org/obo/GAZ_00143785">
        <obo:RO_0001025 rdf:resource="http://purl.obolibrary.org/obo/GAZ_00143783"/>
        <obo:IAO_0000115>One of three plains that comprise the Pacific-Antarctic Basin. It is located at around 100-120degW.</obo:IAO_0000115>
        <oboInOwl:hasOBONamespace>GAZ</oboInOwl:hasOBONamespace>
        <oboInOwl:id>GAZ:00143785</oboInOwl:id>
        <rdfs:label>Bellingshausen Abyssal Plain</rdfs:label>
    </owl:NamedIndividual>
    


    <!-- http://purl.obolibrary.org/obo/GAZ_00143786 -->

    <owl:NamedIndividual rdf:about="http://purl.obolibrary.org/obo/GAZ_00143786">
        <obo:RO_0001025 rdf:resource="http://purl.obolibrary.org/obo/GAZ_00143783"/>
        <obo:IAO_0000115>One of the three plains that comprise the Pacific-Antarctic Basin. It is located at around 150degW.</obo:IAO_0000115>
        <oboInOwl:hasOBONamespace>GAZ</oboInOwl:hasOBONamespace>
        <oboInOwl:id>GAZ:00143786</oboInOwl:id>
        <rdfs:label>Amundsen Abyssal Plain</rdfs:label>
    </owl:NamedIndividual>
    


    <!-- http://purl.obolibrary.org/obo/GAZ_00143787 -->

    <owl:NamedIndividual rdf:about="http://purl.obolibrary.org/obo/GAZ_00143787">
        <obo:RO_0001025 rdf:resource="http://purl.obolibrary.org/obo/GAZ_00000373"/>
        <obo:IAO_0000115>One of three major basins in the Southern Ocean. It extends from its eastern boundary with the Pacific-Antarctic Basin at the longitude of Tasmania (at about 145degE) to the Kerguelan Plateau (at about 75degE). The South-East Indian Ridge separates it from the Indian Ocean at depths greater than 4000 m except for a gap in the Ridge at 117degE.</obo:IAO_0000115>
        <oboInOwl:hasOBONamespace>GAZ</oboInOwl:hasOBONamespace>
        <oboInOwl:id>GAZ:00143787</oboInOwl:id>
        <rdfs:label>Australian-Antarctic Basin</rdfs:label>
    </owl:NamedIndividual>
    


    <!-- http://purl.obolibrary.org/obo/GAZ_00143788 -->

    <owl:NamedIndividual rdf:about="http://purl.obolibrary.org/obo/GAZ_00143788">
        <obo:RO_0001025 rdf:resource="http://purl.obolibrary.org/obo/GAZ_00000373"/>
        <obo:IAO_0000115>A ridge located at approximately 75degE in the Southern Ocean that impedes the flow of the Antarctic Circumpolar Current at depths below 2000 m. Most of this broad plateau is between 2000 and 3000 m deep with some flow occurring below 3000 m in a narrow gap between itself and Antarctica.</obo:IAO_0000115>
        <oboInOwl:hasOBONamespace>GAZ</oboInOwl:hasOBONamespace>
        <oboInOwl:id>GAZ:00143788</oboInOwl:id>
        <rdfs:label>Kerguelan Plateau</rdfs:label>
    </owl:NamedIndividual>
    


    <!-- http://purl.obolibrary.org/obo/GAZ_00143808 -->

    <owl:NamedIndividual rdf:about="http://purl.obolibrary.org/obo/GAZ_00143808">
        <rdf:type rdf:resource="http://purl.obolibrary.org/obo/ENVO_00000084"/>
        <obo:RO_0001025 rdf:resource="http://purl.obolibrary.org/obo/GAZ_00000373"/>
        <obo:IAO_0000115>A gap in the topography between the Kerguelan Plateau and the Antarctic continent, with a sill depth of 3750 m. It provides a route for the exchange of Antarctic Bottom Water (AABW) between the Australian-Antarctic Basin and the Weddell-Enderby Basin.</obo:IAO_0000115>
        <oboInOwl:hasOBONamespace>GAZ</oboInOwl:hasOBONamespace>
        <oboInOwl:id>GAZ:00143808</oboInOwl:id>
        <rdfs:label>Princess Elizabeth Trough</rdfs:label>
    </owl:NamedIndividual>
    


    <!-- http://purl.obolibrary.org/obo/GAZ_00143809 -->

    <owl:NamedIndividual rdf:about="http://purl.obolibrary.org/obo/GAZ_00143809">
        <obo:RO_0001025 rdf:resource="http://purl.obolibrary.org/obo/GAZ_00000373"/>
        <obo:IAO_0000115>A ridge connecting South American and Antarctica located at about 70degW in the Southern Ocean that, along with the narrowing of the Drake Passage 2000 km to the west, impedes the flow of the Antarctic Circumpolar Current (ACC). It is generally less than 2000 m deep with some openings at the 3000 m level.</obo:IAO_0000115>
        <oboInOwl:hasOBONamespace>GAZ</oboInOwl:hasOBONamespace>
        <oboInOwl:id>GAZ:00143809</oboInOwl:id>
        <rdfs:label>Scotia Ridge</rdfs:label>
    </owl:NamedIndividual>
    


    <!-- http://purl.obolibrary.org/obo/GAZ_00228441 -->

    <owl:NamedIndividual rdf:about="http://purl.obolibrary.org/obo/GAZ_00228441">
        <obo:RO_0001025 rdf:resource="http://purl.obolibrary.org/obo/GAZ_00014088"/>
        <obo:IAO_0000115>A subglacial lake in Antarctica. The lake is situated on southern Alexander Island.</obo:IAO_0000115>
        <oboInOwl:hasOBONamespace>GAZ</oboInOwl:hasOBONamespace>
        <oboInOwl:id>GAZ:00228441</oboInOwl:id>
        <rdfs:label>Hodgson Lake</rdfs:label>
    </owl:NamedIndividual>
    


    <!-- http://purl.obolibrary.org/obo/GAZ_00341661 -->

    <owl:NamedIndividual rdf:about="http://purl.obolibrary.org/obo/GAZ_00341661">
        <obo:RO_0001025 rdf:resource="http://purl.obolibrary.org/obo/GAZ_00023352"/>
        <obo:IAO_0000115>An island.</obo:IAO_0000115>
        <oboInOwl:hasOBONamespace>GAZ</oboInOwl:hasOBONamespace>
        <oboInOwl:id>GAZ:00341661</oboInOwl:id>
        <rdfs:label>Ilot de la Balance</rdfs:label>
    </owl:NamedIndividual>
    


    <!-- http://purl.obolibrary.org/obo/GAZ_00341662 -->

    <owl:NamedIndividual rdf:about="http://purl.obolibrary.org/obo/GAZ_00341662">
        <obo:RO_0001025 rdf:resource="http://purl.obolibrary.org/obo/GAZ_00023352"/>
        <obo:IAO_0000115>An island.</obo:IAO_0000115>
        <oboInOwl:hasOBONamespace>GAZ</oboInOwl:hasOBONamespace>
        <oboInOwl:id>GAZ:00341662</oboInOwl:id>
        <rdfs:label>Ilot de la Baleine</rdfs:label>
    </owl:NamedIndividual>
    


    <!-- http://purl.obolibrary.org/obo/GAZ_00341663 -->

    <owl:NamedIndividual rdf:about="http://purl.obolibrary.org/obo/GAZ_00341663">
        <obo:RO_0001025 rdf:resource="http://purl.obolibrary.org/obo/GAZ_00023352"/>
        <obo:IAO_0000115>An island.</obo:IAO_0000115>
        <oboInOwl:hasOBONamespace>GAZ</oboInOwl:hasOBONamespace>
        <oboInOwl:id>GAZ:00341663</oboInOwl:id>
        <rdfs:label>Ile du Belier</rdfs:label>
    </owl:NamedIndividual>
    


    <!-- http://purl.obolibrary.org/obo/GAZ_00341664 -->

    <owl:NamedIndividual rdf:about="http://purl.obolibrary.org/obo/GAZ_00341664">
        <obo:RO_0001025 rdf:resource="http://purl.obolibrary.org/obo/GAZ_00023352"/>
        <obo:IAO_0000115>An island.</obo:IAO_0000115>
        <oboInOwl:hasOBONamespace>GAZ</oboInOwl:hasOBONamespace>
        <oboInOwl:id>GAZ:00341664</oboInOwl:id>
        <rdfs:label>Ile Buffon</rdfs:label>
    </owl:NamedIndividual>
    


    <!-- http://purl.obolibrary.org/obo/GAZ_00341665 -->

    <owl:NamedIndividual rdf:about="http://purl.obolibrary.org/obo/GAZ_00341665">
        <obo:RO_0001025 rdf:resource="http://purl.obolibrary.org/obo/GAZ_00023352"/>
        <obo:IAO_0000115>An island.</obo:IAO_0000115>
        <oboInOwl:hasOBONamespace>GAZ</oboInOwl:hasOBONamespace>
        <oboInOwl:id>GAZ:00341665</oboInOwl:id>
        <rdfs:label>Ilot du Cancer</rdfs:label>
    </owl:NamedIndividual>
    


    <!-- http://purl.obolibrary.org/obo/GAZ_00341666 -->

    <owl:NamedIndividual rdf:about="http://purl.obolibrary.org/obo/GAZ_00341666">
        <obo:RO_0001025 rdf:resource="http://purl.obolibrary.org/obo/GAZ_00023352"/>
        <obo:IAO_0000115>An island.</obo:IAO_0000115>
        <oboInOwl:hasOBONamespace>GAZ</oboInOwl:hasOBONamespace>
        <oboInOwl:id>GAZ:00341666</oboInOwl:id>
        <rdfs:label>Ile du Capricorne</rdfs:label>
    </owl:NamedIndividual>
    


    <!-- http://purl.obolibrary.org/obo/GAZ_00341667 -->

    <owl:NamedIndividual rdf:about="http://purl.obolibrary.org/obo/GAZ_00341667">
        <obo:RO_0001025 rdf:resource="http://purl.obolibrary.org/obo/GAZ_00023352"/>
        <obo:IAO_0000115>An island.</obo:IAO_0000115>
        <oboInOwl:hasOBONamespace>GAZ</oboInOwl:hasOBONamespace>
        <oboInOwl:id>GAZ:00341667</oboInOwl:id>
        <rdfs:label>Ilot des Champignons</rdfs:label>
    </owl:NamedIndividual>
    


    <!-- http://purl.obolibrary.org/obo/GAZ_00341668 -->

    <owl:NamedIndividual rdf:about="http://purl.obolibrary.org/obo/GAZ_00341668">
        <obo:RO_0001025 rdf:resource="http://purl.obolibrary.org/obo/GAZ_00023352"/>
        <obo:IAO_0000115>An island.</obo:IAO_0000115>
        <oboInOwl:hasOBONamespace>GAZ</oboInOwl:hasOBONamespace>
        <oboInOwl:id>GAZ:00341668</oboInOwl:id>
        <rdfs:label>Ile Claude Bernard</rdfs:label>
    </owl:NamedIndividual>
    


    <!-- http://purl.obolibrary.org/obo/GAZ_00341669 -->

    <owl:NamedIndividual rdf:about="http://purl.obolibrary.org/obo/GAZ_00341669">
        <obo:RO_0001025 rdf:resource="http://purl.obolibrary.org/obo/GAZ_00023352"/>
        <obo:IAO_0000115>An island.</obo:IAO_0000115>
        <oboInOwl:hasOBONamespace>GAZ</oboInOwl:hasOBONamespace>
        <oboInOwl:id>GAZ:00341669</oboInOwl:id>
        <rdfs:label>Ile Curie</rdfs:label>
    </owl:NamedIndividual>
    


    <!-- http://purl.obolibrary.org/obo/GAZ_00341670 -->

    <owl:NamedIndividual rdf:about="http://purl.obolibrary.org/obo/GAZ_00341670">
        <obo:RO_0001025 rdf:resource="http://purl.obolibrary.org/obo/GAZ_00023352"/>
        <obo:IAO_0000115>An island.</obo:IAO_0000115>
        <oboInOwl:hasOBONamespace>GAZ</oboInOwl:hasOBONamespace>
        <oboInOwl:id>GAZ:00341670</oboInOwl:id>
        <rdfs:label>Ile des Damiers</rdfs:label>
    </owl:NamedIndividual>
    


    <!-- http://purl.obolibrary.org/obo/GAZ_00341671 -->

    <owl:NamedIndividual rdf:about="http://purl.obolibrary.org/obo/GAZ_00341671">
        <obo:RO_0001025 rdf:resource="http://purl.obolibrary.org/obo/GAZ_00023352"/>
        <obo:IAO_0000115>An island.</obo:IAO_0000115>
        <oboInOwl:hasOBONamespace>GAZ</oboInOwl:hasOBONamespace>
        <oboInOwl:id>GAZ:00341671</oboInOwl:id>
        <rdfs:label>Ilot de la Dent</rdfs:label>
    </owl:NamedIndividual>
    


    <!-- http://purl.obolibrary.org/obo/GAZ_00341672 -->

    <owl:NamedIndividual rdf:about="http://purl.obolibrary.org/obo/GAZ_00341672">
        <obo:RO_0001025 rdf:resource="http://purl.obolibrary.org/obo/GAZ_00023352"/>
        <obo:IAO_0000115>An island.</obo:IAO_0000115>
        <oboInOwl:hasOBONamespace>GAZ</oboInOwl:hasOBONamespace>
        <oboInOwl:id>GAZ:00341672</oboInOwl:id>
        <rdfs:label>Ile du Gouverneur</rdfs:label>
    </owl:NamedIndividual>
    


    <!-- http://purl.obolibrary.org/obo/GAZ_00341673 -->

    <owl:NamedIndividual rdf:about="http://purl.obolibrary.org/obo/GAZ_00341673">
        <obo:RO_0001025 rdf:resource="http://purl.obolibrary.org/obo/GAZ_00023352"/>
        <obo:IAO_0000115>An island.</obo:IAO_0000115>
        <oboInOwl:hasOBONamespace>GAZ</oboInOwl:hasOBONamespace>
        <oboInOwl:id>GAZ:00341673</oboInOwl:id>
        <rdfs:label>Rocher Gris</rdfs:label>
    </owl:NamedIndividual>
    


    <!-- http://purl.obolibrary.org/obo/GAZ_00341674 -->

    <owl:NamedIndividual rdf:about="http://purl.obolibrary.org/obo/GAZ_00341674">
        <obo:RO_0001025 rdf:resource="http://purl.obolibrary.org/obo/GAZ_00023352"/>
        <obo:IAO_0000115>An island.</obo:IAO_0000115>
        <oboInOwl:hasOBONamespace>GAZ</oboInOwl:hasOBONamespace>
        <oboInOwl:id>GAZ:00341674</oboInOwl:id>
        <rdfs:label>Ilots des Hydrographes</rdfs:label>
    </owl:NamedIndividual>
    


    <!-- http://purl.obolibrary.org/obo/GAZ_00341675 -->

    <owl:NamedIndividual rdf:about="http://purl.obolibrary.org/obo/GAZ_00341675">
        <obo:RO_0001025 rdf:resource="http://purl.obolibrary.org/obo/GAZ_00023352"/>
        <obo:IAO_0000115>An island.</obo:IAO_0000115>
        <oboInOwl:hasOBONamespace>GAZ</oboInOwl:hasOBONamespace>
        <oboInOwl:id>GAZ:00341675</oboInOwl:id>
        <rdfs:label>Ilot Juliette</rdfs:label>
    </owl:NamedIndividual>
    


    <!-- http://purl.obolibrary.org/obo/GAZ_00341676 -->

    <owl:NamedIndividual rdf:about="http://purl.obolibrary.org/obo/GAZ_00341676">
        <obo:RO_0001025 rdf:resource="http://purl.obolibrary.org/obo/GAZ_00023352"/>
        <obo:IAO_0000115>An island.</obo:IAO_0000115>
        <oboInOwl:hasOBONamespace>GAZ</oboInOwl:hasOBONamespace>
        <oboInOwl:id>GAZ:00341676</oboInOwl:id>
        <rdfs:label>Ile Lamarck</rdfs:label>
    </owl:NamedIndividual>
    


    <!-- http://purl.obolibrary.org/obo/GAZ_00341677 -->

    <owl:NamedIndividual rdf:about="http://purl.obolibrary.org/obo/GAZ_00341677">
        <obo:RO_0001025 rdf:resource="http://purl.obolibrary.org/obo/GAZ_00023352"/>
        <obo:IAO_0000115>An island.</obo:IAO_0000115>
        <oboInOwl:hasOBONamespace>GAZ</oboInOwl:hasOBONamespace>
        <oboInOwl:id>GAZ:00341677</oboInOwl:id>
        <rdfs:label>Le Mauguen</rdfs:label>
    </owl:NamedIndividual>
    


    <!-- http://purl.obolibrary.org/obo/GAZ_00341678 -->

    <owl:NamedIndividual rdf:about="http://purl.obolibrary.org/obo/GAZ_00341678">
        <obo:RO_0001025 rdf:resource="http://purl.obolibrary.org/obo/GAZ_00023352"/>
        <obo:IAO_0000115>An island.</obo:IAO_0000115>
        <oboInOwl:hasOBONamespace>GAZ</oboInOwl:hasOBONamespace>
        <oboInOwl:id>GAZ:00341678</oboInOwl:id>
        <rdfs:label>Mid-Winter</rdfs:label>
    </owl:NamedIndividual>
    


    <!-- http://purl.obolibrary.org/obo/GAZ_00341679 -->

    <owl:NamedIndividual rdf:about="http://purl.obolibrary.org/obo/GAZ_00341679">
        <obo:RO_0001025 rdf:resource="http://purl.obolibrary.org/obo/GAZ_00023352"/>
        <obo:IAO_0000115>An island.</obo:IAO_0000115>
        <oboInOwl:hasOBONamespace>GAZ</oboInOwl:hasOBONamespace>
        <oboInOwl:id>GAZ:00341679</oboInOwl:id>
        <rdfs:label>Ilot du Mystere</rdfs:label>
    </owl:NamedIndividual>
    


    <!-- http://purl.obolibrary.org/obo/GAZ_00341680 -->

    <owl:NamedIndividual rdf:about="http://purl.obolibrary.org/obo/GAZ_00341680">
        <obo:RO_0001025 rdf:resource="http://purl.obolibrary.org/obo/GAZ_00023352"/>
        <obo:IAO_0000115>An island.</obo:IAO_0000115>
        <oboInOwl:hasOBONamespace>GAZ</oboInOwl:hasOBONamespace>
        <oboInOwl:id>GAZ:00341680</oboInOwl:id>
        <rdfs:label>Ile du Navigateur</rdfs:label>
    </owl:NamedIndividual>
    


    <!-- http://purl.obolibrary.org/obo/GAZ_00341681 -->

    <owl:NamedIndividual rdf:about="http://purl.obolibrary.org/obo/GAZ_00341681">
        <obo:RO_0001025 rdf:resource="http://purl.obolibrary.org/obo/GAZ_00023352"/>
        <obo:IAO_0000115>An island.</obo:IAO_0000115>
        <oboInOwl:hasOBONamespace>GAZ</oboInOwl:hasOBONamespace>
        <oboInOwl:id>GAZ:00341681</oboInOwl:id>
        <rdfs:label>Iles des Poissons</rdfs:label>
    </owl:NamedIndividual>
    


    <!-- http://purl.obolibrary.org/obo/GAZ_00341682 -->

    <owl:NamedIndividual rdf:about="http://purl.obolibrary.org/obo/GAZ_00341682">
        <obo:RO_0001025 rdf:resource="http://purl.obolibrary.org/obo/GAZ_00023352"/>
        <obo:IAO_0000115>An island.</obo:IAO_0000115>
        <oboInOwl:hasOBONamespace>GAZ</oboInOwl:hasOBONamespace>
        <oboInOwl:id>GAZ:00341682</oboInOwl:id>
        <rdfs:label>Ilot Romeo</rdfs:label>
    </owl:NamedIndividual>
    


    <!-- http://purl.obolibrary.org/obo/GAZ_00341683 -->

    <owl:NamedIndividual rdf:about="http://purl.obolibrary.org/obo/GAZ_00341683">
        <obo:RO_0001025 rdf:resource="http://purl.obolibrary.org/obo/GAZ_00023352"/>
        <obo:IAO_0000115>An island.</obo:IAO_0000115>
        <oboInOwl:hasOBONamespace>GAZ</oboInOwl:hasOBONamespace>
        <oboInOwl:id>GAZ:00341683</oboInOwl:id>
        <rdfs:label>Ile du Sagittaire</rdfs:label>
    </owl:NamedIndividual>
    


    <!-- http://purl.obolibrary.org/obo/GAZ_00341684 -->

    <owl:NamedIndividual rdf:about="http://purl.obolibrary.org/obo/GAZ_00341684">
        <obo:RO_0001025 rdf:resource="http://purl.obolibrary.org/obo/GAZ_00023352"/>
        <obo:IAO_0000115>An island.</obo:IAO_0000115>
        <oboInOwl:hasOBONamespace>GAZ</oboInOwl:hasOBONamespace>
        <oboInOwl:id>GAZ:00341684</oboInOwl:id>
        <rdfs:label>Ile du Scorpion</rdfs:label>
    </owl:NamedIndividual>
    


    <!-- http://purl.obolibrary.org/obo/GAZ_00341685 -->

    <owl:NamedIndividual rdf:about="http://purl.obolibrary.org/obo/GAZ_00341685">
        <obo:RO_0001025 rdf:resource="http://purl.obolibrary.org/obo/GAZ_00023352"/>
        <obo:IAO_0000115>An island.</obo:IAO_0000115>
        <oboInOwl:hasOBONamespace>GAZ</oboInOwl:hasOBONamespace>
        <oboInOwl:id>GAZ:00341685</oboInOwl:id>
        <rdfs:label>Ilot de la Selle</rdfs:label>
    </owl:NamedIndividual>
    


    <!-- http://purl.obolibrary.org/obo/GAZ_00341686 -->

    <owl:NamedIndividual rdf:about="http://purl.obolibrary.org/obo/GAZ_00341686">
        <obo:RO_0001025 rdf:resource="http://purl.obolibrary.org/obo/GAZ_00023352"/>
        <obo:IAO_0000115>An island.</obo:IAO_0000115>
        <oboInOwl:hasOBONamespace>GAZ</oboInOwl:hasOBONamespace>
        <oboInOwl:id>GAZ:00341686</oboInOwl:id>
        <rdfs:label>Ile du Taureau</rdfs:label>
    </owl:NamedIndividual>
    


    <!-- http://purl.obolibrary.org/obo/GAZ_00341687 -->

    <owl:NamedIndividual rdf:about="http://purl.obolibrary.org/obo/GAZ_00341687">
        <obo:RO_0001025 rdf:resource="http://purl.obolibrary.org/obo/GAZ_00023352"/>
        <obo:IAO_0000115>An island.</obo:IAO_0000115>
        <oboInOwl:hasOBONamespace>GAZ</oboInOwl:hasOBONamespace>
        <oboInOwl:id>GAZ:00341687</oboInOwl:id>
        <rdfs:label>Ilot du Verseau</rdfs:label>
    </owl:NamedIndividual>
    


    <!-- http://purl.obolibrary.org/obo/GAZ_00341688 -->

    <owl:NamedIndividual rdf:about="http://purl.obolibrary.org/obo/GAZ_00341688">
        <obo:RO_0001025 rdf:resource="http://purl.obolibrary.org/obo/GAZ_00023352"/>
        <obo:IAO_0000115>An island.</obo:IAO_0000115>
        <oboInOwl:hasOBONamespace>GAZ</oboInOwl:hasOBONamespace>
        <oboInOwl:id>GAZ:00341688</oboInOwl:id>
        <rdfs:label>Ile de la Vierge</rdfs:label>
    </owl:NamedIndividual>
    


    <!-- http://purl.obolibrary.org/obo/GAZ_00447311 -->

    <owl:NamedIndividual rdf:about="http://purl.obolibrary.org/obo/GAZ_00447311">
        <obo:RO_0001025 rdf:resource="http://purl.obolibrary.org/obo/GAZ_00023348"/>
        <obo:IAO_0000115>An area of hydrothermal vents.</obo:IAO_0000115>
        <oboInOwl:hasOBONamespace>GAZ</oboInOwl:hasOBONamespace>
        <oboInOwl:id>GAZ:00447311</oboInOwl:id>
        <rdfs:label>Hook Ridge</rdfs:label>
    </owl:NamedIndividual>
    


    <!-- http://purl.obolibrary.org/obo/GAZ_01000004 -->

    <owl:NamedIndividual rdf:about="http://purl.obolibrary.org/obo/GAZ_01000004">
        <obo:RO_0001025 rdf:resource="http://purl.obolibrary.org/obo/GAZ_00000373"/>
    </owl:NamedIndividual>
    


    <!-- 
    ///////////////////////////////////////////////////////////////////////////////////////
    //
    // Annotations
    //
    ///////////////////////////////////////////////////////////////////////////////////////
     -->

    <rdf:Description rdf:about="http://purl.obolibrary.org/obo/GAZ_00000373">
        <rdfs:label>Southern Ocean</rdfs:label>
        <oboInOwl:hasOBONamespace>GAZ</oboInOwl:hasOBONamespace>
        <obo:IAO_0000115>The oceanic division completely in Earth&apos;s southern hemisphere encircling Antarctica, comprising the southernmost waters of the World Ocean south of 60degS latitude. However, the Southern Ocean&apos;s northern boundary is not precise. Instead, the Antarctic Convergence, an ocean zone which fluctuates seasonally, separates the Southern Ocean from other oceans. This dynamic, natural boundary is formed by the convergence of two circumpolar currents, one easterly flowing and one westerly.</obo:IAO_0000115>
        <oboInOwl:id>GAZ:00000373</oboInOwl:id>
    </rdf:Description>
    <rdf:Description rdf:about="http://purl.obolibrary.org/obo/GAZ_00014125">
        <oboInOwl:hasOBONamespace>GAZ</oboInOwl:hasOBONamespace>
        <rdfs:label>ANDEEP station</rdfs:label>
        <oboInOwl:id>GAZ:00014125</oboInOwl:id>
        <obo:IAO_0000115>AnDEEP: ANtarctic benthic DEEP sea biodiversity: colonization history and recent community patterns (An international project to investigate the deep-water biology of the Scotia and Weddell seas from F/S Polarstern).</obo:IAO_0000115>
    </rdf:Description>
    <rdf:Description rdf:about="http://purl.obolibrary.org/obo/GAZ_01000004">
        <oboInOwl:id>GAZ:01000004</oboInOwl:id>
        <oboInOwl:hasOBONamespace>GAZ</oboInOwl:hasOBONamespace>
        <rdfs:label>Southern Ocean Current</rdfs:label>
    </rdf:Description>
</rdf:RDF>



<!-- Generated by the OWL API (version 4.5.6) https://github.com/owlcs/owlapi -->

