<?xml version="1.0"?>
<rdf:RDF xmlns="http://purl.obolibrary.org/obo/gaz/subsets/countries/Afghanistan.owl#"
     xml:base="http://purl.obolibrary.org/obo/gaz/subsets/countries/Afghanistan.owl"
     xmlns:obo="http://purl.obolibrary.org/obo/"
     xmlns:owl="http://www.w3.org/2002/07/owl#"
     xmlns:rdf="http://www.w3.org/1999/02/22-rdf-syntax-ns#"
     xmlns:xml="http://www.w3.org/XML/1998/namespace"
     xmlns:xsd="http://www.w3.org/2001/XMLSchema#"
     xmlns:rdfs="http://www.w3.org/2000/01/rdf-schema#"
     xmlns:oboInOwl="http://www.geneontology.org/formats/oboInOwl#">
    <owl:Ontology rdf:about="http://purl.obolibrary.org/obo/gaz/subsets/countries/Afghanistan.owl">
        <owl:imports rdf:resource="http://purl.obolibrary.org/obo/gaz/imports/envo_import.owl"/>
        <owl:imports rdf:resource="http://purl.obolibrary.org/obo/gaz/imports/ro_import.owl"/>
    </owl:Ontology>
    


    <!-- 
    ///////////////////////////////////////////////////////////////////////////////////////
    //
    // Annotation properties
    //
    ///////////////////////////////////////////////////////////////////////////////////////
     -->

    


    <!-- http://purl.obolibrary.org/obo/IAO_0000115 -->

    <owl:AnnotationProperty rdf:about="http://purl.obolibrary.org/obo/IAO_0000115"/>
    


    <!-- http://www.geneontology.org/formats/oboInOwl#hasOBONamespace -->

    <owl:AnnotationProperty rdf:about="http://www.geneontology.org/formats/oboInOwl#hasOBONamespace"/>
    


    <!-- http://www.geneontology.org/formats/oboInOwl#id -->

    <owl:AnnotationProperty rdf:about="http://www.geneontology.org/formats/oboInOwl#id"/>
    


    <!-- 
    ///////////////////////////////////////////////////////////////////////////////////////
    //
    // Object Properties
    //
    ///////////////////////////////////////////////////////////////////////////////////////
     -->

    


    <!-- http://purl.obolibrary.org/obo/RO_0001025 -->

    <owl:ObjectProperty rdf:about="http://purl.obolibrary.org/obo/RO_0001025"/>
    


    <!-- 
    ///////////////////////////////////////////////////////////////////////////////////////
    //
    // Classes
    //
    ///////////////////////////////////////////////////////////////////////////////////////
     -->

    


    <!-- http://purl.obolibrary.org/obo/ENVO_00000004 -->

    <owl:Class rdf:about="http://purl.obolibrary.org/obo/ENVO_00000004"/>
    


    <!-- http://purl.obolibrary.org/obo/ENVO_00000074 -->

    <owl:Class rdf:about="http://purl.obolibrary.org/obo/ENVO_00000074"/>
    


    <!-- http://purl.obolibrary.org/obo/ENVO_00000104 -->

    <owl:Class rdf:about="http://purl.obolibrary.org/obo/ENVO_00000104"/>
    


    <!-- http://purl.obolibrary.org/obo/ENVO_00000106 -->

    <owl:Class rdf:about="http://purl.obolibrary.org/obo/ENVO_00000106"/>
    


    <!-- http://purl.obolibrary.org/obo/ENVO_00000354 -->

    <owl:Class rdf:about="http://purl.obolibrary.org/obo/ENVO_00000354"/>
    


    <!-- http://purl.obolibrary.org/obo/ENVO_00000856 -->

    <owl:Class rdf:about="http://purl.obolibrary.org/obo/ENVO_00000856"/>
    


    <!-- http://purl.obolibrary.org/obo/GAZ_00009461 -->

    <owl:Class rdf:about="http://purl.obolibrary.org/obo/GAZ_00009461"/>
    


    <!-- http://purl.obolibrary.org/obo/GAZ_00010626 -->

    <owl:Class rdf:about="http://purl.obolibrary.org/obo/GAZ_00010626">
        <rdfs:subClassOf rdf:resource="http://purl.obolibrary.org/obo/GAZ_00009461"/>
    </owl:Class>
    


    <!-- http://purl.obolibrary.org/obo/GAZ_00010627 -->

    <owl:Class rdf:about="http://purl.obolibrary.org/obo/GAZ_00010627">
        <rdfs:subClassOf rdf:resource="http://purl.obolibrary.org/obo/GAZ_00009461"/>
    </owl:Class>
    


    <!-- http://purl.obolibrary.org/obo/GAZ_00010628 -->

    <owl:Class rdf:about="http://purl.obolibrary.org/obo/GAZ_00010628">
        <rdfs:subClassOf rdf:resource="http://purl.obolibrary.org/obo/GAZ_00009461"/>
    </owl:Class>
    


    <!-- http://purl.obolibrary.org/obo/GAZ_00010629 -->

    <owl:Class rdf:about="http://purl.obolibrary.org/obo/GAZ_00010629">
        <rdfs:subClassOf rdf:resource="http://purl.obolibrary.org/obo/GAZ_00009461"/>
    </owl:Class>
    


    <!-- http://purl.obolibrary.org/obo/GAZ_00010630 -->

    <owl:Class rdf:about="http://purl.obolibrary.org/obo/GAZ_00010630">
        <rdfs:subClassOf rdf:resource="http://purl.obolibrary.org/obo/GAZ_00009461"/>
    </owl:Class>
    


    <!-- http://purl.obolibrary.org/obo/GAZ_00010631 -->

    <owl:Class rdf:about="http://purl.obolibrary.org/obo/GAZ_00010631">
        <rdfs:subClassOf rdf:resource="http://purl.obolibrary.org/obo/GAZ_00009461"/>
    </owl:Class>
    


    <!-- http://purl.obolibrary.org/obo/GAZ_00010632 -->

    <owl:Class rdf:about="http://purl.obolibrary.org/obo/GAZ_00010632">
        <rdfs:subClassOf rdf:resource="http://purl.obolibrary.org/obo/GAZ_00009461"/>
    </owl:Class>
    


    <!-- http://purl.obolibrary.org/obo/GAZ_00010633 -->

    <owl:Class rdf:about="http://purl.obolibrary.org/obo/GAZ_00010633">
        <rdfs:subClassOf rdf:resource="http://purl.obolibrary.org/obo/GAZ_00009461"/>
    </owl:Class>
    


    <!-- http://purl.obolibrary.org/obo/GAZ_00010634 -->

    <owl:Class rdf:about="http://purl.obolibrary.org/obo/GAZ_00010634">
        <rdfs:subClassOf rdf:resource="http://purl.obolibrary.org/obo/GAZ_00009461"/>
    </owl:Class>
    


    <!-- http://purl.obolibrary.org/obo/GAZ_00010635 -->

    <owl:Class rdf:about="http://purl.obolibrary.org/obo/GAZ_00010635">
        <rdfs:subClassOf rdf:resource="http://purl.obolibrary.org/obo/GAZ_00009461"/>
    </owl:Class>
    


    <!-- http://purl.obolibrary.org/obo/GAZ_00010636 -->

    <owl:Class rdf:about="http://purl.obolibrary.org/obo/GAZ_00010636">
        <rdfs:subClassOf rdf:resource="http://purl.obolibrary.org/obo/GAZ_00009461"/>
    </owl:Class>
    


    <!-- http://purl.obolibrary.org/obo/GAZ_00010637 -->

    <owl:Class rdf:about="http://purl.obolibrary.org/obo/GAZ_00010637">
        <rdfs:subClassOf rdf:resource="http://purl.obolibrary.org/obo/GAZ_00009461"/>
    </owl:Class>
    


    <!-- http://purl.obolibrary.org/obo/GAZ_00010638 -->

    <owl:Class rdf:about="http://purl.obolibrary.org/obo/GAZ_00010638">
        <rdfs:subClassOf rdf:resource="http://purl.obolibrary.org/obo/GAZ_00009461"/>
    </owl:Class>
    


    <!-- http://purl.obolibrary.org/obo/GAZ_00010639 -->

    <owl:Class rdf:about="http://purl.obolibrary.org/obo/GAZ_00010639">
        <rdfs:subClassOf rdf:resource="http://purl.obolibrary.org/obo/GAZ_00009461"/>
    </owl:Class>
    


    <!-- http://purl.obolibrary.org/obo/GAZ_00010640 -->

    <owl:Class rdf:about="http://purl.obolibrary.org/obo/GAZ_00010640">
        <rdfs:subClassOf rdf:resource="http://purl.obolibrary.org/obo/GAZ_00009461"/>
    </owl:Class>
    


    <!-- http://purl.obolibrary.org/obo/GAZ_00010641 -->

    <owl:Class rdf:about="http://purl.obolibrary.org/obo/GAZ_00010641">
        <rdfs:subClassOf rdf:resource="http://purl.obolibrary.org/obo/GAZ_00009461"/>
    </owl:Class>
    


    <!-- http://purl.obolibrary.org/obo/GAZ_00010642 -->

    <owl:Class rdf:about="http://purl.obolibrary.org/obo/GAZ_00010642">
        <rdfs:subClassOf rdf:resource="http://purl.obolibrary.org/obo/GAZ_00009461"/>
    </owl:Class>
    


    <!-- http://purl.obolibrary.org/obo/GAZ_00010643 -->

    <owl:Class rdf:about="http://purl.obolibrary.org/obo/GAZ_00010643">
        <rdfs:subClassOf rdf:resource="http://purl.obolibrary.org/obo/GAZ_00009461"/>
    </owl:Class>
    


    <!-- http://purl.obolibrary.org/obo/GAZ_00010644 -->

    <owl:Class rdf:about="http://purl.obolibrary.org/obo/GAZ_00010644">
        <rdfs:subClassOf rdf:resource="http://purl.obolibrary.org/obo/GAZ_00009461"/>
    </owl:Class>
    


    <!-- http://purl.obolibrary.org/obo/GAZ_00010645 -->

    <owl:Class rdf:about="http://purl.obolibrary.org/obo/GAZ_00010645">
        <rdfs:subClassOf rdf:resource="http://purl.obolibrary.org/obo/GAZ_00009461"/>
    </owl:Class>
    


    <!-- http://purl.obolibrary.org/obo/GAZ_00010646 -->

    <owl:Class rdf:about="http://purl.obolibrary.org/obo/GAZ_00010646">
        <rdfs:subClassOf rdf:resource="http://purl.obolibrary.org/obo/GAZ_00009461"/>
    </owl:Class>
    


    <!-- http://purl.obolibrary.org/obo/GAZ_00010647 -->

    <owl:Class rdf:about="http://purl.obolibrary.org/obo/GAZ_00010647">
        <rdfs:subClassOf rdf:resource="http://purl.obolibrary.org/obo/GAZ_00009461"/>
    </owl:Class>
    


    <!-- http://purl.obolibrary.org/obo/GAZ_00010648 -->

    <owl:Class rdf:about="http://purl.obolibrary.org/obo/GAZ_00010648">
        <rdfs:subClassOf rdf:resource="http://purl.obolibrary.org/obo/GAZ_00009461"/>
    </owl:Class>
    


    <!-- http://purl.obolibrary.org/obo/GAZ_00010649 -->

    <owl:Class rdf:about="http://purl.obolibrary.org/obo/GAZ_00010649">
        <rdfs:subClassOf rdf:resource="http://purl.obolibrary.org/obo/GAZ_00009461"/>
    </owl:Class>
    


    <!-- http://purl.obolibrary.org/obo/GAZ_00010650 -->

    <owl:Class rdf:about="http://purl.obolibrary.org/obo/GAZ_00010650">
        <rdfs:subClassOf rdf:resource="http://purl.obolibrary.org/obo/GAZ_00009461"/>
    </owl:Class>
    


    <!-- http://purl.obolibrary.org/obo/GAZ_00010651 -->

    <owl:Class rdf:about="http://purl.obolibrary.org/obo/GAZ_00010651">
        <rdfs:subClassOf rdf:resource="http://purl.obolibrary.org/obo/GAZ_00009461"/>
    </owl:Class>
    


    <!-- http://purl.obolibrary.org/obo/GAZ_00010652 -->

    <owl:Class rdf:about="http://purl.obolibrary.org/obo/GAZ_00010652">
        <rdfs:subClassOf rdf:resource="http://purl.obolibrary.org/obo/GAZ_00009461"/>
    </owl:Class>
    


    <!-- http://purl.obolibrary.org/obo/GAZ_00010653 -->

    <owl:Class rdf:about="http://purl.obolibrary.org/obo/GAZ_00010653">
        <rdfs:subClassOf rdf:resource="http://purl.obolibrary.org/obo/GAZ_00009461"/>
    </owl:Class>
    


    <!-- http://purl.obolibrary.org/obo/GAZ_00010654 -->

    <owl:Class rdf:about="http://purl.obolibrary.org/obo/GAZ_00010654">
        <rdfs:subClassOf rdf:resource="http://purl.obolibrary.org/obo/GAZ_00009461"/>
    </owl:Class>
    


    <!-- http://purl.obolibrary.org/obo/GAZ_00010655 -->

    <owl:Class rdf:about="http://purl.obolibrary.org/obo/GAZ_00010655">
        <rdfs:subClassOf rdf:resource="http://purl.obolibrary.org/obo/GAZ_00009461"/>
    </owl:Class>
    


    <!-- http://purl.obolibrary.org/obo/GAZ_00010656 -->

    <owl:Class rdf:about="http://purl.obolibrary.org/obo/GAZ_00010656">
        <rdfs:subClassOf rdf:resource="http://purl.obolibrary.org/obo/GAZ_00009461"/>
    </owl:Class>
    


    <!-- http://purl.obolibrary.org/obo/GAZ_00010657 -->

    <owl:Class rdf:about="http://purl.obolibrary.org/obo/GAZ_00010657">
        <rdfs:subClassOf rdf:resource="http://purl.obolibrary.org/obo/GAZ_00009461"/>
    </owl:Class>
    


    <!-- http://purl.obolibrary.org/obo/GAZ_00010658 -->

    <owl:Class rdf:about="http://purl.obolibrary.org/obo/GAZ_00010658">
        <rdfs:subClassOf rdf:resource="http://purl.obolibrary.org/obo/GAZ_00009461"/>
    </owl:Class>
    


    <!-- http://purl.obolibrary.org/obo/GAZ_00010659 -->

    <owl:Class rdf:about="http://purl.obolibrary.org/obo/GAZ_00010659">
        <rdfs:subClassOf rdf:resource="http://purl.obolibrary.org/obo/GAZ_00009461"/>
    </owl:Class>
    


    <!-- 
    ///////////////////////////////////////////////////////////////////////////////////////
    //
    // Individuals
    //
    ///////////////////////////////////////////////////////////////////////////////////////
     -->

    


    <!-- http://purl.obolibrary.org/obo/GAZ_00004988 -->

    <owl:NamedIndividual rdf:about="http://purl.obolibrary.org/obo/GAZ_00004988">
        <obo:RO_0001025 rdf:resource="http://purl.obolibrary.org/obo/GAZ_00006882"/>
        <obo:IAO_0000115>A mountain range located in Central Asia and are formed by the junction or knot of the Tian Shan, Karakoram, Kunlun, and Hindu Kush ranges. The Pamir region is centered in the Tajikistani region of Gorno-Badakhshan. Parts of the Pamir also lie in the countries of Kyrgyzstan, Afghanistan, and Pakistan. South of Gorno-Badakhshan, the Wakhan Corridor runs through the Pamir region, which also includes the northern extremes of the North-West Frontier Province and the northern extremes of the Northern Areas of Pakistan.</obo:IAO_0000115>
        <oboInOwl:hasOBONamespace>GAZ</oboInOwl:hasOBONamespace>
        <oboInOwl:id>GAZ:00004988</oboInOwl:id>
        <rdfs:label>Pamir Mountains</rdfs:label>
    </owl:NamedIndividual>
    


    <!-- http://purl.obolibrary.org/obo/GAZ_00006882 -->

    <owl:NamedIndividual rdf:about="http://purl.obolibrary.org/obo/GAZ_00006882">
        <obo:IAO_0000115>A landlocked country that is located approximately in the center of Asia. It is bordered by Pakistan in the south and east Iran in the west, Turkmenistan, Uzbekistan and Tajikistan in the north, and China in the far northeast. Afghanistan is administratively divided into thirty-four (34) provinces (welayats). Each province is then divided into many provincial districts, and each district normally covers a city or several townships.</obo:IAO_0000115>
        <oboInOwl:hasOBONamespace>GAZ</oboInOwl:hasOBONamespace>
        <oboInOwl:id>GAZ:00006882</oboInOwl:id>
        <rdfs:label>Afghanistan</rdfs:label>
    </owl:NamedIndividual>
    


    <!-- http://purl.obolibrary.org/obo/GAZ_00008310 -->

    <owl:NamedIndividual rdf:about="http://purl.obolibrary.org/obo/GAZ_00008310">
        <obo:RO_0001025 rdf:resource="http://purl.obolibrary.org/obo/GAZ_00004988"/>
        <oboInOwl:hasOBONamespace>GAZ</oboInOwl:hasOBONamespace>
        <oboInOwl:id>GAZ:00008310</oboInOwl:id>
        <rdfs:label>East Pamirs</rdfs:label>
    </owl:NamedIndividual>
    


    <!-- http://purl.obolibrary.org/obo/GAZ_00009461 -->

    <owl:NamedIndividual rdf:about="http://purl.obolibrary.org/obo/GAZ_00009461">
        <obo:RO_0001025 rdf:resource="http://purl.obolibrary.org/obo/GAZ_00006882"/>
    </owl:NamedIndividual>
    


    <!-- http://purl.obolibrary.org/obo/GAZ_00010626 -->

    <owl:NamedIndividual rdf:about="http://purl.obolibrary.org/obo/GAZ_00010626"/>
    


    <!-- http://purl.obolibrary.org/obo/GAZ_00010627 -->

    <owl:NamedIndividual rdf:about="http://purl.obolibrary.org/obo/GAZ_00010627"/>
    


    <!-- http://purl.obolibrary.org/obo/GAZ_00010628 -->

    <owl:NamedIndividual rdf:about="http://purl.obolibrary.org/obo/GAZ_00010628"/>
    


    <!-- http://purl.obolibrary.org/obo/GAZ_00010629 -->

    <owl:NamedIndividual rdf:about="http://purl.obolibrary.org/obo/GAZ_00010629"/>
    


    <!-- http://purl.obolibrary.org/obo/GAZ_00010630 -->

    <owl:NamedIndividual rdf:about="http://purl.obolibrary.org/obo/GAZ_00010630"/>
    


    <!-- http://purl.obolibrary.org/obo/GAZ_00010631 -->

    <owl:NamedIndividual rdf:about="http://purl.obolibrary.org/obo/GAZ_00010631"/>
    


    <!-- http://purl.obolibrary.org/obo/GAZ_00010632 -->

    <owl:NamedIndividual rdf:about="http://purl.obolibrary.org/obo/GAZ_00010632"/>
    


    <!-- http://purl.obolibrary.org/obo/GAZ_00010633 -->

    <owl:NamedIndividual rdf:about="http://purl.obolibrary.org/obo/GAZ_00010633"/>
    


    <!-- http://purl.obolibrary.org/obo/GAZ_00010634 -->

    <owl:NamedIndividual rdf:about="http://purl.obolibrary.org/obo/GAZ_00010634"/>
    


    <!-- http://purl.obolibrary.org/obo/GAZ_00010635 -->

    <owl:NamedIndividual rdf:about="http://purl.obolibrary.org/obo/GAZ_00010635"/>
    


    <!-- http://purl.obolibrary.org/obo/GAZ_00010636 -->

    <owl:NamedIndividual rdf:about="http://purl.obolibrary.org/obo/GAZ_00010636"/>
    


    <!-- http://purl.obolibrary.org/obo/GAZ_00010637 -->

    <owl:NamedIndividual rdf:about="http://purl.obolibrary.org/obo/GAZ_00010637"/>
    


    <!-- http://purl.obolibrary.org/obo/GAZ_00010638 -->

    <owl:NamedIndividual rdf:about="http://purl.obolibrary.org/obo/GAZ_00010638"/>
    


    <!-- http://purl.obolibrary.org/obo/GAZ_00010639 -->

    <owl:NamedIndividual rdf:about="http://purl.obolibrary.org/obo/GAZ_00010639"/>
    


    <!-- http://purl.obolibrary.org/obo/GAZ_00010640 -->

    <owl:NamedIndividual rdf:about="http://purl.obolibrary.org/obo/GAZ_00010640"/>
    


    <!-- http://purl.obolibrary.org/obo/GAZ_00010641 -->

    <owl:NamedIndividual rdf:about="http://purl.obolibrary.org/obo/GAZ_00010641"/>
    


    <!-- http://purl.obolibrary.org/obo/GAZ_00010642 -->

    <owl:NamedIndividual rdf:about="http://purl.obolibrary.org/obo/GAZ_00010642"/>
    


    <!-- http://purl.obolibrary.org/obo/GAZ_00010643 -->

    <owl:NamedIndividual rdf:about="http://purl.obolibrary.org/obo/GAZ_00010643"/>
    


    <!-- http://purl.obolibrary.org/obo/GAZ_00010644 -->

    <owl:NamedIndividual rdf:about="http://purl.obolibrary.org/obo/GAZ_00010644"/>
    


    <!-- http://purl.obolibrary.org/obo/GAZ_00010645 -->

    <owl:NamedIndividual rdf:about="http://purl.obolibrary.org/obo/GAZ_00010645"/>
    


    <!-- http://purl.obolibrary.org/obo/GAZ_00010646 -->

    <owl:NamedIndividual rdf:about="http://purl.obolibrary.org/obo/GAZ_00010646"/>
    


    <!-- http://purl.obolibrary.org/obo/GAZ_00010647 -->

    <owl:NamedIndividual rdf:about="http://purl.obolibrary.org/obo/GAZ_00010647"/>
    


    <!-- http://purl.obolibrary.org/obo/GAZ_00010648 -->

    <owl:NamedIndividual rdf:about="http://purl.obolibrary.org/obo/GAZ_00010648"/>
    


    <!-- http://purl.obolibrary.org/obo/GAZ_00010649 -->

    <owl:NamedIndividual rdf:about="http://purl.obolibrary.org/obo/GAZ_00010649"/>
    


    <!-- http://purl.obolibrary.org/obo/GAZ_00010650 -->

    <owl:NamedIndividual rdf:about="http://purl.obolibrary.org/obo/GAZ_00010650"/>
    


    <!-- http://purl.obolibrary.org/obo/GAZ_00010651 -->

    <owl:NamedIndividual rdf:about="http://purl.obolibrary.org/obo/GAZ_00010651"/>
    


    <!-- http://purl.obolibrary.org/obo/GAZ_00010652 -->

    <owl:NamedIndividual rdf:about="http://purl.obolibrary.org/obo/GAZ_00010652"/>
    


    <!-- http://purl.obolibrary.org/obo/GAZ_00010653 -->

    <owl:NamedIndividual rdf:about="http://purl.obolibrary.org/obo/GAZ_00010653"/>
    


    <!-- http://purl.obolibrary.org/obo/GAZ_00010654 -->

    <owl:NamedIndividual rdf:about="http://purl.obolibrary.org/obo/GAZ_00010654"/>
    


    <!-- http://purl.obolibrary.org/obo/GAZ_00010655 -->

    <owl:NamedIndividual rdf:about="http://purl.obolibrary.org/obo/GAZ_00010655"/>
    


    <!-- http://purl.obolibrary.org/obo/GAZ_00010656 -->

    <owl:NamedIndividual rdf:about="http://purl.obolibrary.org/obo/GAZ_00010656"/>
    


    <!-- http://purl.obolibrary.org/obo/GAZ_00010657 -->

    <owl:NamedIndividual rdf:about="http://purl.obolibrary.org/obo/GAZ_00010657"/>
    


    <!-- http://purl.obolibrary.org/obo/GAZ_00010658 -->

    <owl:NamedIndividual rdf:about="http://purl.obolibrary.org/obo/GAZ_00010658"/>
    


    <!-- http://purl.obolibrary.org/obo/GAZ_00010659 -->

    <owl:NamedIndividual rdf:about="http://purl.obolibrary.org/obo/GAZ_00010659"/>
    


    <!-- http://purl.obolibrary.org/obo/GAZ_00011784 -->

    <owl:NamedIndividual rdf:about="http://purl.obolibrary.org/obo/GAZ_00011784">
        <obo:RO_0001025 rdf:resource="http://purl.obolibrary.org/obo/GAZ_00057344"/>
        <obo:IAO_0000115>A mountain of the Himalaya range in High Asia, is located on the border between Nepal and Tibet, China.</obo:IAO_0000115>
        <oboInOwl:hasOBONamespace>GAZ</oboInOwl:hasOBONamespace>
        <oboInOwl:id>GAZ:00011784</oboInOwl:id>
        <rdfs:label>Mount Everest</rdfs:label>
    </owl:NamedIndividual>
    


    <!-- http://purl.obolibrary.org/obo/GAZ_00013531 -->

    <owl:NamedIndividual rdf:about="http://purl.obolibrary.org/obo/GAZ_00013531">
        <obo:RO_0001025 rdf:resource="http://purl.obolibrary.org/obo/GAZ_00021571"/>
        <obo:IAO_0000115>A populated place. in Nawur District.</obo:IAO_0000115>
        <oboInOwl:hasOBONamespace>GAZ</oboInOwl:hasOBONamespace>
        <oboInOwl:id>GAZ:00013531</oboInOwl:id>
        <rdfs:label>Okak</rdfs:label>
    </owl:NamedIndividual>
    


    <!-- http://purl.obolibrary.org/obo/GAZ_00021436 -->

    <owl:NamedIndividual rdf:about="http://purl.obolibrary.org/obo/GAZ_00021436">
        <rdf:type rdf:resource="http://purl.obolibrary.org/obo/ENVO_00000004"/>
        <obo:RO_0001025 rdf:resource="http://purl.obolibrary.org/obo/GAZ_00010651"/>
        <obo:IAO_0000115>A district of Badakhshan Province, Afghanistan. Its northwestern border is along the international border between Afghanistan and Tajikistan while its southwestern border is with Takhar Province.</obo:IAO_0000115>
        <oboInOwl:hasOBONamespace>GAZ</oboInOwl:hasOBONamespace>
        <oboInOwl:id>GAZ:00021436</oboInOwl:id>
        <rdfs:label>Shahri Buzurg District</rdfs:label>
    </owl:NamedIndividual>
    


    <!-- http://purl.obolibrary.org/obo/GAZ_00021482 -->

    <owl:NamedIndividual rdf:about="http://purl.obolibrary.org/obo/GAZ_00021482">
        <rdf:type rdf:resource="http://purl.obolibrary.org/obo/ENVO_00000004"/>
        <obo:RO_0001025 rdf:resource="http://purl.obolibrary.org/obo/GAZ_00010651"/>
        <obo:IAO_0000115>A district of Badakhshan Province in eastern Afghanistan.</obo:IAO_0000115>
        <oboInOwl:hasOBONamespace>GAZ</oboInOwl:hasOBONamespace>
        <oboInOwl:id>GAZ:00021482</oboInOwl:id>
        <rdfs:label>Zebak District</rdfs:label>
    </owl:NamedIndividual>
    


    <!-- http://purl.obolibrary.org/obo/GAZ_00021483 -->

    <owl:NamedIndividual rdf:about="http://purl.obolibrary.org/obo/GAZ_00021483">
        <rdf:type rdf:resource="http://purl.obolibrary.org/obo/ENVO_00000004"/>
        <obo:RO_0001025 rdf:resource="http://purl.obolibrary.org/obo/GAZ_00010651"/>
        <obo:IAO_0000115>A district of Badakhshan Province, Afghanistan. The district is in the southwest corner of the province, and is bordered on its northeast side by Jurm and Zebak Districts. Most of the rest of the district&apos;s boundaries are adjacent to other Afghan provinces, but a very small section on the eastern edge of the district lies on the international border between Afghanistan and Pakistan.</obo:IAO_0000115>
        <oboInOwl:hasOBONamespace>GAZ</oboInOwl:hasOBONamespace>
        <oboInOwl:id>GAZ:00021483</oboInOwl:id>
        <rdfs:label>Kuran Wa Munjan District</rdfs:label>
    </owl:NamedIndividual>
    


    <!-- http://purl.obolibrary.org/obo/GAZ_00021484 -->

    <owl:NamedIndividual rdf:about="http://purl.obolibrary.org/obo/GAZ_00021484">
        <rdf:type rdf:resource="http://purl.obolibrary.org/obo/ENVO_00000004"/>
        <obo:RO_0001025 rdf:resource="http://purl.obolibrary.org/obo/GAZ_00010651"/>
        <obo:IAO_0000115>A district of Badakhshan Province, Afghanistan.</obo:IAO_0000115>
        <oboInOwl:hasOBONamespace>GAZ</oboInOwl:hasOBONamespace>
        <oboInOwl:id>GAZ:00021484</oboInOwl:id>
        <rdfs:label>Jurm District</rdfs:label>
    </owl:NamedIndividual>
    


    <!-- http://purl.obolibrary.org/obo/GAZ_00021485 -->

    <owl:NamedIndividual rdf:about="http://purl.obolibrary.org/obo/GAZ_00021485">
        <rdf:type rdf:resource="http://purl.obolibrary.org/obo/ENVO_00000004"/>
        <obo:RO_0001025 rdf:resource="http://purl.obolibrary.org/obo/GAZ_00010651"/>
        <obo:IAO_0000115>A district of Badakhshan Province, Afghanistan.</obo:IAO_0000115>
        <oboInOwl:hasOBONamespace>GAZ</oboInOwl:hasOBONamespace>
        <oboInOwl:id>GAZ:00021485</oboInOwl:id>
        <rdfs:label>Khwahan District</rdfs:label>
    </owl:NamedIndividual>
    


    <!-- http://purl.obolibrary.org/obo/GAZ_00021486 -->

    <owl:NamedIndividual rdf:about="http://purl.obolibrary.org/obo/GAZ_00021486">
        <rdf:type rdf:resource="http://purl.obolibrary.org/obo/ENVO_00000004"/>
        <obo:RO_0001025 rdf:resource="http://purl.obolibrary.org/obo/GAZ_00010651"/>
        <obo:IAO_0000115>A district of Badakhshan Province, Afghanistan.</obo:IAO_0000115>
        <oboInOwl:hasOBONamespace>GAZ</oboInOwl:hasOBONamespace>
        <oboInOwl:id>GAZ:00021486</oboInOwl:id>
        <rdfs:label>Kishim District</rdfs:label>
    </owl:NamedIndividual>
    


    <!-- http://purl.obolibrary.org/obo/GAZ_00021487 -->

    <owl:NamedIndividual rdf:about="http://purl.obolibrary.org/obo/GAZ_00021487">
        <rdf:type rdf:resource="http://purl.obolibrary.org/obo/ENVO_00000004"/>
        <obo:RO_0001025 rdf:resource="http://purl.obolibrary.org/obo/GAZ_00010651"/>
        <obo:IAO_0000115>A district of Badakhshan Province, Afghanistan.</obo:IAO_0000115>
        <oboInOwl:hasOBONamespace>GAZ</oboInOwl:hasOBONamespace>
        <oboInOwl:id>GAZ:00021487</oboInOwl:id>
        <rdfs:label>Shighnan District</rdfs:label>
    </owl:NamedIndividual>
    


    <!-- http://purl.obolibrary.org/obo/GAZ_00021488 -->

    <owl:NamedIndividual rdf:about="http://purl.obolibrary.org/obo/GAZ_00021488">
        <rdf:type rdf:resource="http://purl.obolibrary.org/obo/ENVO_00000004"/>
        <obo:RO_0001025 rdf:resource="http://purl.obolibrary.org/obo/GAZ_00010651"/>
        <obo:IAO_0000115>A district of Badakhshan Province, Afghanistan.</obo:IAO_0000115>
        <oboInOwl:hasOBONamespace>GAZ</oboInOwl:hasOBONamespace>
        <oboInOwl:id>GAZ:00021488</oboInOwl:id>
        <rdfs:label>Ragh District</rdfs:label>
    </owl:NamedIndividual>
    


    <!-- http://purl.obolibrary.org/obo/GAZ_00021489 -->

    <owl:NamedIndividual rdf:about="http://purl.obolibrary.org/obo/GAZ_00021489">
        <rdf:type rdf:resource="http://purl.obolibrary.org/obo/ENVO_00000004"/>
        <obo:RO_0001025 rdf:resource="http://purl.obolibrary.org/obo/GAZ_00010651"/>
        <obo:IAO_0000115>A district of Badakhshan Province, Afghanistan.</obo:IAO_0000115>
        <oboInOwl:hasOBONamespace>GAZ</oboInOwl:hasOBONamespace>
        <oboInOwl:id>GAZ:00021489</oboInOwl:id>
        <rdfs:label>Ishkashim District</rdfs:label>
    </owl:NamedIndividual>
    


    <!-- http://purl.obolibrary.org/obo/GAZ_00021490 -->

    <owl:NamedIndividual rdf:about="http://purl.obolibrary.org/obo/GAZ_00021490">
        <rdf:type rdf:resource="http://purl.obolibrary.org/obo/ENVO_00000004"/>
        <obo:RO_0001025 rdf:resource="http://purl.obolibrary.org/obo/GAZ_00010651"/>
        <obo:IAO_0000115>A district of Badakhshan Province, Afghanistan. In 2005, several portions of the district were sub-divided to create several new districts within the province.</obo:IAO_0000115>
        <oboInOwl:hasOBONamespace>GAZ</oboInOwl:hasOBONamespace>
        <oboInOwl:id>GAZ:00021490</oboInOwl:id>
        <rdfs:label>Fayzabad District</rdfs:label>
    </owl:NamedIndividual>
    


    <!-- http://purl.obolibrary.org/obo/GAZ_00021491 -->

    <owl:NamedIndividual rdf:about="http://purl.obolibrary.org/obo/GAZ_00021491">
        <rdf:type rdf:resource="http://purl.obolibrary.org/obo/ENVO_00000004"/>
        <obo:RO_0001025 rdf:resource="http://purl.obolibrary.org/obo/GAZ_00098853"/>
        <obo:IAO_0000115>A district in Badakhshan Province, Afghanistan.</obo:IAO_0000115>
        <oboInOwl:hasOBONamespace>GAZ</oboInOwl:hasOBONamespace>
        <oboInOwl:id>GAZ:00021491</oboInOwl:id>
        <rdfs:label>Wakhan District</rdfs:label>
    </owl:NamedIndividual>
    


    <!-- http://purl.obolibrary.org/obo/GAZ_00021492 -->

    <owl:NamedIndividual rdf:about="http://purl.obolibrary.org/obo/GAZ_00021492">
        <rdf:type rdf:resource="http://purl.obolibrary.org/obo/ENVO_00000004"/>
        <obo:RO_0001025 rdf:resource="http://purl.obolibrary.org/obo/GAZ_00010651"/>
        <obo:IAO_0000115>A district of Badakhshan Province, Afghanistan located east from Fayzabad.</obo:IAO_0000115>
        <oboInOwl:hasOBONamespace>GAZ</oboInOwl:hasOBONamespace>
        <oboInOwl:id>GAZ:00021492</oboInOwl:id>
        <rdfs:label>Baharak District</rdfs:label>
    </owl:NamedIndividual>
    


    <!-- http://purl.obolibrary.org/obo/GAZ_00021493 -->

    <owl:NamedIndividual rdf:about="http://purl.obolibrary.org/obo/GAZ_00021493">
        <rdf:type rdf:resource="http://purl.obolibrary.org/obo/ENVO_00000004"/>
        <obo:RO_0001025 rdf:resource="http://purl.obolibrary.org/obo/GAZ_00010651"/>
        <obo:IAO_0000115>A district in the province of Badakhshan in Afghanistan.</obo:IAO_0000115>
        <oboInOwl:hasOBONamespace>GAZ</oboInOwl:hasOBONamespace>
        <oboInOwl:id>GAZ:00021493</oboInOwl:id>
        <rdfs:label>Darwaz District</rdfs:label>
    </owl:NamedIndividual>
    


    <!-- http://purl.obolibrary.org/obo/GAZ_00021494 -->

    <owl:NamedIndividual rdf:about="http://purl.obolibrary.org/obo/GAZ_00021494">
        <rdf:type rdf:resource="http://purl.obolibrary.org/obo/ENVO_00000004"/>
        <obo:RO_0001025 rdf:resource="http://purl.obolibrary.org/obo/GAZ_00010658"/>
        <obo:IAO_0000115>A district located in the southern part of Badghis province, Afghanistan, between the districts Jawand in the East, Qala i Naw in the west, Muqur and Murghab in the North. In the South is the Herat province.</obo:IAO_0000115>
        <oboInOwl:hasOBONamespace>GAZ</oboInOwl:hasOBONamespace>
        <oboInOwl:id>GAZ:00021494</oboInOwl:id>
        <rdfs:label>Qadis District</rdfs:label>
    </owl:NamedIndividual>
    


    <!-- http://purl.obolibrary.org/obo/GAZ_00021495 -->

    <owl:NamedIndividual rdf:about="http://purl.obolibrary.org/obo/GAZ_00021495">
        <rdf:type rdf:resource="http://purl.obolibrary.org/obo/ENVO_00000004"/>
        <obo:RO_0001025 rdf:resource="http://purl.obolibrary.org/obo/GAZ_00010658"/>
        <obo:IAO_0000115>A district of Badghis Province, in the western part of Afghanistan. It is located between the districts of Ab Kamari to the east, Qala i Naw to the south, Qadis to the southeast and Murghab to the northeast. To the north is the national border with Turkmenistan.</obo:IAO_0000115>
        <oboInOwl:hasOBONamespace>GAZ</oboInOwl:hasOBONamespace>
        <oboInOwl:id>GAZ:00021495</oboInOwl:id>
        <rdfs:label>Muqur District</rdfs:label>
    </owl:NamedIndividual>
    


    <!-- http://purl.obolibrary.org/obo/GAZ_00021496 -->

    <owl:NamedIndividual rdf:about="http://purl.obolibrary.org/obo/GAZ_00021496">
        <rdf:type rdf:resource="http://purl.obolibrary.org/obo/ENVO_00000004"/>
        <obo:RO_0001025 rdf:resource="http://purl.obolibrary.org/obo/GAZ_00010658"/>
        <obo:IAO_0000115>A district in the west of Badghis Province, Afghanistan.</obo:IAO_0000115>
        <oboInOwl:hasOBONamespace>GAZ</oboInOwl:hasOBONamespace>
        <oboInOwl:id>GAZ:00021496</oboInOwl:id>
        <rdfs:label>Qala-I-Naw District</rdfs:label>
    </owl:NamedIndividual>
    


    <!-- http://purl.obolibrary.org/obo/GAZ_00021497 -->

    <owl:NamedIndividual rdf:about="http://purl.obolibrary.org/obo/GAZ_00021497">
        <obo:RO_0001025 rdf:resource="http://purl.obolibrary.org/obo/GAZ_00010658"/>
        <obo:IAO_0000115>The largest district of Badghis Province, Afghanistan, located in the southeast.</obo:IAO_0000115>
        <oboInOwl:hasOBONamespace>GAZ</oboInOwl:hasOBONamespace>
        <oboInOwl:id>GAZ:00021497</oboInOwl:id>
        <rdfs:label>Jawand District</rdfs:label>
    </owl:NamedIndividual>
    


    <!-- http://purl.obolibrary.org/obo/GAZ_00021498 -->

    <owl:NamedIndividual rdf:about="http://purl.obolibrary.org/obo/GAZ_00021498">
        <rdf:type rdf:resource="http://purl.obolibrary.org/obo/ENVO_00000004"/>
        <obo:RO_0001025 rdf:resource="http://purl.obolibrary.org/obo/GAZ_00010658"/>
        <obo:IAO_0000115>A district in the west of Badghis Province, Afghanistan.</obo:IAO_0000115>
        <oboInOwl:hasOBONamespace>GAZ</oboInOwl:hasOBONamespace>
        <oboInOwl:id>GAZ:00021498</oboInOwl:id>
        <rdfs:label>Ab Kamari District</rdfs:label>
    </owl:NamedIndividual>
    


    <!-- http://purl.obolibrary.org/obo/GAZ_00021499 -->

    <owl:NamedIndividual rdf:about="http://purl.obolibrary.org/obo/GAZ_00021499">
        <rdf:type rdf:resource="http://purl.obolibrary.org/obo/ENVO_00000004"/>
        <obo:RO_0001025 rdf:resource="http://purl.obolibrary.org/obo/GAZ_00010658"/>
        <obo:IAO_0000115>A district in the north of Badghis Province, Afghanistan. To the west, it borders on Turkmenistan.</obo:IAO_0000115>
        <oboInOwl:hasOBONamespace>GAZ</oboInOwl:hasOBONamespace>
        <oboInOwl:id>GAZ:00021499</oboInOwl:id>
        <rdfs:label>Murghab District</rdfs:label>
    </owl:NamedIndividual>
    


    <!-- http://purl.obolibrary.org/obo/GAZ_00021500 -->

    <owl:NamedIndividual rdf:about="http://purl.obolibrary.org/obo/GAZ_00021500">
        <rdf:type rdf:resource="http://purl.obolibrary.org/obo/ENVO_00000004"/>
        <obo:RO_0001025 rdf:resource="http://purl.obolibrary.org/obo/GAZ_00010658"/>
        <obo:IAO_0000115>A district in northeast Badghis Province, Afghanistan. It borders on Turkmenistan to the north, the Almar and Qaysar districts of Faryab Province to the east, and Murghab District to the south and to the west.</obo:IAO_0000115>
        <oboInOwl:hasOBONamespace>GAZ</oboInOwl:hasOBONamespace>
        <oboInOwl:id>GAZ:00021500</oboInOwl:id>
        <rdfs:label>Ghormach District</rdfs:label>
    </owl:NamedIndividual>
    


    <!-- http://purl.obolibrary.org/obo/GAZ_00021501 -->

    <owl:NamedIndividual rdf:about="http://purl.obolibrary.org/obo/GAZ_00021501">
        <rdf:type rdf:resource="http://purl.obolibrary.org/obo/ENVO_00000004"/>
        <obo:RO_0001025 rdf:resource="http://purl.obolibrary.org/obo/GAZ_00010659"/>
        <obo:IAO_0000115>A district in the northeastern part of Baghlan province.</obo:IAO_0000115>
        <oboInOwl:hasOBONamespace>GAZ</oboInOwl:hasOBONamespace>
        <oboInOwl:id>GAZ:00021501</oboInOwl:id>
        <rdfs:label>Burka District</rdfs:label>
    </owl:NamedIndividual>
    


    <!-- http://purl.obolibrary.org/obo/GAZ_00021502 -->

    <owl:NamedIndividual rdf:about="http://purl.obolibrary.org/obo/GAZ_00021502">
        <rdf:type rdf:resource="http://purl.obolibrary.org/obo/ENVO_00000004"/>
        <obo:RO_0001025 rdf:resource="http://purl.obolibrary.org/obo/GAZ_00010659"/>
        <obo:IAO_0000115>A district in Baghlan Province, Afghanistan.</obo:IAO_0000115>
        <oboInOwl:hasOBONamespace>GAZ</oboInOwl:hasOBONamespace>
        <oboInOwl:id>GAZ:00021502</oboInOwl:id>
        <rdfs:label>Baghlan District</rdfs:label>
    </owl:NamedIndividual>
    


    <!-- http://purl.obolibrary.org/obo/GAZ_00021503 -->

    <owl:NamedIndividual rdf:about="http://purl.obolibrary.org/obo/GAZ_00021503">
        <rdf:type rdf:resource="http://purl.obolibrary.org/obo/ENVO_00000004"/>
        <obo:RO_0001025 rdf:resource="http://purl.obolibrary.org/obo/GAZ_00010659"/>
        <obo:IAO_0000115>A district of Afghanistan situated in the most southwestern part of Baghlan province.</obo:IAO_0000115>
        <oboInOwl:hasOBONamespace>GAZ</oboInOwl:hasOBONamespace>
        <oboInOwl:id>GAZ:00021503</oboInOwl:id>
        <rdfs:label>Tala Wa Barfak District</rdfs:label>
    </owl:NamedIndividual>
    


    <!-- http://purl.obolibrary.org/obo/GAZ_00021504 -->

    <owl:NamedIndividual rdf:about="http://purl.obolibrary.org/obo/GAZ_00021504">
        <rdf:type rdf:resource="http://purl.obolibrary.org/obo/ENVO_00000004"/>
        <obo:RO_0001025 rdf:resource="http://purl.obolibrary.org/obo/GAZ_00010659"/>
        <obo:IAO_0000115>A district located in the most southwestern part of Baghlan province.</obo:IAO_0000115>
        <oboInOwl:hasOBONamespace>GAZ</oboInOwl:hasOBONamespace>
        <oboInOwl:id>GAZ:00021504</oboInOwl:id>
        <rdfs:label>Dahana-I-Ghori District</rdfs:label>
    </owl:NamedIndividual>
    


    <!-- http://purl.obolibrary.org/obo/GAZ_00021505 -->

    <owl:NamedIndividual rdf:about="http://purl.obolibrary.org/obo/GAZ_00021505">
        <rdf:type rdf:resource="http://purl.obolibrary.org/obo/ENVO_00000004"/>
        <obo:RO_0001025 rdf:resource="http://purl.obolibrary.org/obo/GAZ_00010659"/>
        <obo:IAO_0000115>A district of Baghlan Province, Afghanistan. It is situated in the northern-most part of the province, just north of Baghlan district, and borders to the north on Kunduz Province and to the west on Samangan Province.</obo:IAO_0000115>
        <oboInOwl:hasOBONamespace>GAZ</oboInOwl:hasOBONamespace>
        <oboInOwl:id>GAZ:00021505</oboInOwl:id>
        <rdfs:label>Baghlani Jadid District</rdfs:label>
    </owl:NamedIndividual>
    


    <!-- http://purl.obolibrary.org/obo/GAZ_00021506 -->

    <owl:NamedIndividual rdf:about="http://purl.obolibrary.org/obo/GAZ_00021506">
        <rdf:type rdf:resource="http://purl.obolibrary.org/obo/ENVO_00000004"/>
        <obo:RO_0001025 rdf:resource="http://purl.obolibrary.org/obo/GAZ_00010659"/>
        <obo:IAO_0000115>A district located in the central part of the Baghlan province, south from the Puli Khumri district.</obo:IAO_0000115>
        <oboInOwl:hasOBONamespace>GAZ</oboInOwl:hasOBONamespace>
        <oboInOwl:id>GAZ:00021506</oboInOwl:id>
        <rdfs:label>Dushi District</rdfs:label>
    </owl:NamedIndividual>
    


    <!-- http://purl.obolibrary.org/obo/GAZ_00021507 -->

    <owl:NamedIndividual rdf:about="http://purl.obolibrary.org/obo/GAZ_00021507">
        <rdf:type rdf:resource="http://purl.obolibrary.org/obo/ENVO_00000004"/>
        <obo:RO_0001025 rdf:resource="http://purl.obolibrary.org/obo/GAZ_00010657"/>
        <obo:IAO_0000115>A district of Bamiyan province in central Afghanistan. It was part of Baghlan Province in the past, but in 2005, part of the district was split off to form Sayghan district.</obo:IAO_0000115>
        <oboInOwl:hasOBONamespace>GAZ</oboInOwl:hasOBONamespace>
        <oboInOwl:id>GAZ:00021507</oboInOwl:id>
        <rdfs:label>Kahmard District</rdfs:label>
    </owl:NamedIndividual>
    


    <!-- http://purl.obolibrary.org/obo/GAZ_00021508 -->

    <owl:NamedIndividual rdf:about="http://purl.obolibrary.org/obo/GAZ_00021508">
        <rdf:type rdf:resource="http://purl.obolibrary.org/obo/ENVO_00000004"/>
        <obo:RO_0001025 rdf:resource="http://purl.obolibrary.org/obo/GAZ_00010659"/>
        <obo:IAO_0000115>A district of Afghanistan situated in the Baghlan province.</obo:IAO_0000115>
        <oboInOwl:hasOBONamespace>GAZ</oboInOwl:hasOBONamespace>
        <oboInOwl:id>GAZ:00021508</oboInOwl:id>
        <rdfs:label>Puli Khumri District</rdfs:label>
    </owl:NamedIndividual>
    


    <!-- http://purl.obolibrary.org/obo/GAZ_00021509 -->

    <owl:NamedIndividual rdf:about="http://purl.obolibrary.org/obo/GAZ_00021509">
        <obo:RO_0001025 rdf:resource="http://purl.obolibrary.org/obo/GAZ_00010659"/>
        <obo:IAO_0000115>The most Eastern district of Baghlan province, Afghanistan, in the Hindu Kush mountains.</obo:IAO_0000115>
        <oboInOwl:hasOBONamespace>GAZ</oboInOwl:hasOBONamespace>
        <oboInOwl:id>GAZ:00021509</oboInOwl:id>
        <rdfs:label>Khost Wa Firing District</rdfs:label>
    </owl:NamedIndividual>
    


    <!-- http://purl.obolibrary.org/obo/GAZ_00021510 -->

    <owl:NamedIndividual rdf:about="http://purl.obolibrary.org/obo/GAZ_00021510">
        <rdf:type rdf:resource="http://purl.obolibrary.org/obo/ENVO_00000004"/>
        <obo:RO_0001025 rdf:resource="http://purl.obolibrary.org/obo/GAZ_00010659"/>
        <obo:IAO_0000115>A district located in the southern part of Baghlan province in the Hindu Kush mountains.</obo:IAO_0000115>
        <oboInOwl:hasOBONamespace>GAZ</oboInOwl:hasOBONamespace>
        <oboInOwl:id>GAZ:00021510</oboInOwl:id>
        <rdfs:label>Khinjan District</rdfs:label>
    </owl:NamedIndividual>
    


    <!-- http://purl.obolibrary.org/obo/GAZ_00021511 -->

    <owl:NamedIndividual rdf:about="http://purl.obolibrary.org/obo/GAZ_00021511">
        <rdf:type rdf:resource="http://purl.obolibrary.org/obo/ENVO_00000004"/>
        <obo:RO_0001025 rdf:resource="http://purl.obolibrary.org/obo/GAZ_00010659"/>
        <obo:IAO_0000115>A district in the southern part of Baghlan province in the northeastern Afghanistan.</obo:IAO_0000115>
        <oboInOwl:hasOBONamespace>GAZ</oboInOwl:hasOBONamespace>
        <oboInOwl:id>GAZ:00021511</oboInOwl:id>
        <rdfs:label>Andarab District</rdfs:label>
    </owl:NamedIndividual>
    


    <!-- http://purl.obolibrary.org/obo/GAZ_00021512 -->

    <owl:NamedIndividual rdf:about="http://purl.obolibrary.org/obo/GAZ_00021512">
        <rdf:type rdf:resource="http://purl.obolibrary.org/obo/ENVO_00000004"/>
        <obo:RO_0001025 rdf:resource="http://purl.obolibrary.org/obo/GAZ_00010659"/>
        <obo:IAO_0000115>A district in the central part of Baghlan Province in Afghanistan.</obo:IAO_0000115>
        <oboInOwl:hasOBONamespace>GAZ</oboInOwl:hasOBONamespace>
        <oboInOwl:id>GAZ:00021512</oboInOwl:id>
        <rdfs:label>Nahrin District</rdfs:label>
    </owl:NamedIndividual>
    


    <!-- http://purl.obolibrary.org/obo/GAZ_00021513 -->

    <owl:NamedIndividual rdf:about="http://purl.obolibrary.org/obo/GAZ_00021513">
        <rdf:type rdf:resource="http://purl.obolibrary.org/obo/ENVO_00000004"/>
        <obo:RO_0001025 rdf:resource="http://purl.obolibrary.org/obo/GAZ_00010654"/>
        <obo:IAO_0000115>A district located in the northwestern part of Balkh province in Afghanistan.</obo:IAO_0000115>
        <oboInOwl:hasOBONamespace>GAZ</oboInOwl:hasOBONamespace>
        <oboInOwl:id>GAZ:00021513</oboInOwl:id>
        <rdfs:label>Dawlatabad District</rdfs:label>
    </owl:NamedIndividual>
    


    <!-- http://purl.obolibrary.org/obo/GAZ_00021514 -->

    <owl:NamedIndividual rdf:about="http://purl.obolibrary.org/obo/GAZ_00021514">
        <rdf:type rdf:resource="http://purl.obolibrary.org/obo/ENVO_00000004"/>
        <obo:RO_0001025 rdf:resource="http://purl.obolibrary.org/obo/GAZ_00010654"/>
        <obo:IAO_0000115>A district in Balkh Province, Afghanistan.</obo:IAO_0000115>
        <oboInOwl:hasOBONamespace>GAZ</oboInOwl:hasOBONamespace>
        <oboInOwl:id>GAZ:00021514</oboInOwl:id>
        <rdfs:label>Balkh District</rdfs:label>
    </owl:NamedIndividual>
    


    <!-- http://purl.obolibrary.org/obo/GAZ_00021515 -->

    <owl:NamedIndividual rdf:about="http://purl.obolibrary.org/obo/GAZ_00021515">
        <rdf:type rdf:resource="http://purl.obolibrary.org/obo/ENVO_00000004"/>
        <obo:RO_0001025 rdf:resource="http://purl.obolibrary.org/obo/GAZ_00010654"/>
        <obo:IAO_0000115>A small district in Balkh Province, Afghanistan. It is situated along the Amu Darya river, close to the border with Uzbekistan.</obo:IAO_0000115>
        <oboInOwl:hasOBONamespace>GAZ</oboInOwl:hasOBONamespace>
        <oboInOwl:id>GAZ:00021515</oboInOwl:id>
        <rdfs:label>Shortepa District</rdfs:label>
    </owl:NamedIndividual>
    


    <!-- http://purl.obolibrary.org/obo/GAZ_00021516 -->

    <owl:NamedIndividual rdf:about="http://purl.obolibrary.org/obo/GAZ_00021516">
        <rdf:type rdf:resource="http://purl.obolibrary.org/obo/ENVO_00000004"/>
        <obo:RO_0001025 rdf:resource="http://purl.obolibrary.org/obo/GAZ_00010654"/>
        <obo:IAO_0000115>A district in Balkh Province of Afghanistan.</obo:IAO_0000115>
        <oboInOwl:hasOBONamespace>GAZ</oboInOwl:hasOBONamespace>
        <oboInOwl:id>GAZ:00021516</oboInOwl:id>
        <rdfs:label>Chahar Kint District</rdfs:label>
    </owl:NamedIndividual>
    


    <!-- http://purl.obolibrary.org/obo/GAZ_00021517 -->

    <owl:NamedIndividual rdf:about="http://purl.obolibrary.org/obo/GAZ_00021517">
        <rdf:type rdf:resource="http://purl.obolibrary.org/obo/ENVO_00000004"/>
        <obo:RO_0001025 rdf:resource="http://purl.obolibrary.org/obo/GAZ_00010654"/>
        <obo:IAO_0000115>A district located in the central part of Balkh province in Northern Afghanistan.</obo:IAO_0000115>
        <oboInOwl:hasOBONamespace>GAZ</oboInOwl:hasOBONamespace>
        <oboInOwl:id>GAZ:00021517</oboInOwl:id>
        <rdfs:label>Dihdadi District</rdfs:label>
    </owl:NamedIndividual>
    


    <!-- http://purl.obolibrary.org/obo/GAZ_00021518 -->

    <owl:NamedIndividual rdf:about="http://purl.obolibrary.org/obo/GAZ_00021518">
        <rdf:type rdf:resource="http://purl.obolibrary.org/obo/ENVO_00000004"/>
        <obo:RO_0001025 rdf:resource="http://purl.obolibrary.org/obo/GAZ_00010654"/>
        <obo:IAO_0000115>A district located in the western part of Balkh province, Afghanistan.</obo:IAO_0000115>
        <oboInOwl:hasOBONamespace>GAZ</oboInOwl:hasOBONamespace>
        <oboInOwl:id>GAZ:00021518</oboInOwl:id>
        <rdfs:label>Chimtal District</rdfs:label>
    </owl:NamedIndividual>
    


    <!-- http://purl.obolibrary.org/obo/GAZ_00021519 -->

    <owl:NamedIndividual rdf:about="http://purl.obolibrary.org/obo/GAZ_00021519">
        <rdf:type rdf:resource="http://purl.obolibrary.org/obo/ENVO_00000004"/>
        <obo:RO_0001025 rdf:resource="http://purl.obolibrary.org/obo/GAZ_00010654"/>
        <obo:IAO_0000115>A district of Balkh Province, Afghanistan.</obo:IAO_0000115>
        <oboInOwl:hasOBONamespace>GAZ</oboInOwl:hasOBONamespace>
        <oboInOwl:id>GAZ:00021519</oboInOwl:id>
        <rdfs:label>Nahri Shahi District</rdfs:label>
    </owl:NamedIndividual>
    


    <!-- http://purl.obolibrary.org/obo/GAZ_00021520 -->

    <owl:NamedIndividual rdf:about="http://purl.obolibrary.org/obo/GAZ_00021520">
        <obo:RO_0001025 rdf:resource="http://purl.obolibrary.org/obo/GAZ_00010654"/>
        <obo:IAO_0000115>The most southern district in Balkh province.</obo:IAO_0000115>
        <oboInOwl:hasOBONamespace>GAZ</oboInOwl:hasOBONamespace>
        <oboInOwl:id>GAZ:00021520</oboInOwl:id>
        <rdfs:label>Kishindih District</rdfs:label>
    </owl:NamedIndividual>
    


    <!-- http://purl.obolibrary.org/obo/GAZ_00021521 -->

    <owl:NamedIndividual rdf:about="http://purl.obolibrary.org/obo/GAZ_00021521">
        <rdf:type rdf:resource="http://purl.obolibrary.org/obo/ENVO_00000004"/>
        <obo:RO_0001025 rdf:resource="http://purl.obolibrary.org/obo/GAZ_00010654"/>
        <obo:IAO_0000115>A district located in the western part of Balkh province.</obo:IAO_0000115>
        <oboInOwl:hasOBONamespace>GAZ</oboInOwl:hasOBONamespace>
        <oboInOwl:id>GAZ:00021521</oboInOwl:id>
        <rdfs:label>Chahar Bolak District</rdfs:label>
    </owl:NamedIndividual>
    


    <!-- http://purl.obolibrary.org/obo/GAZ_00021522 -->

    <owl:NamedIndividual rdf:about="http://purl.obolibrary.org/obo/GAZ_00021522">
        <rdf:type rdf:resource="http://purl.obolibrary.org/obo/ENVO_00000004"/>
        <obo:RO_0001025 rdf:resource="http://purl.obolibrary.org/obo/GAZ_00010654"/>
        <obo:IAO_0000115>A district located in the central part of the Balkh province.</obo:IAO_0000115>
        <oboInOwl:hasOBONamespace>GAZ</oboInOwl:hasOBONamespace>
        <oboInOwl:id>GAZ:00021522</oboInOwl:id>
        <rdfs:label>Marmul District</rdfs:label>
    </owl:NamedIndividual>
    


    <!-- http://purl.obolibrary.org/obo/GAZ_00021523 -->

    <owl:NamedIndividual rdf:about="http://purl.obolibrary.org/obo/GAZ_00021523">
        <rdf:type rdf:resource="http://purl.obolibrary.org/obo/ENVO_00000004"/>
        <obo:RO_0001025 rdf:resource="http://purl.obolibrary.org/obo/GAZ_00010654"/>
        <obo:IAO_0000115>A district located in the northern part of Balkh Province, Afghanistan. The northern and the eastern border of the district is the large Amu Darya river. North of the river is Uzbekistan and in the East is Tajikistan.</obo:IAO_0000115>
        <oboInOwl:hasOBONamespace>GAZ</oboInOwl:hasOBONamespace>
        <oboInOwl:id>GAZ:00021523</oboInOwl:id>
        <rdfs:label>Kaldar District</rdfs:label>
    </owl:NamedIndividual>
    


    <!-- http://purl.obolibrary.org/obo/GAZ_00021524 -->

    <owl:NamedIndividual rdf:about="http://purl.obolibrary.org/obo/GAZ_00021524">
        <rdf:type rdf:resource="http://purl.obolibrary.org/obo/ENVO_00000004"/>
        <obo:RO_0001025 rdf:resource="http://purl.obolibrary.org/obo/GAZ_00010654"/>
        <obo:IAO_0000115>A district of Balkh Province in Afghanistan.</obo:IAO_0000115>
        <oboInOwl:hasOBONamespace>GAZ</oboInOwl:hasOBONamespace>
        <oboInOwl:id>GAZ:00021524</oboInOwl:id>
        <rdfs:label>Mazar-I-Sharif District</rdfs:label>
    </owl:NamedIndividual>
    


    <!-- http://purl.obolibrary.org/obo/GAZ_00021525 -->

    <owl:NamedIndividual rdf:about="http://purl.obolibrary.org/obo/GAZ_00021525">
        <rdf:type rdf:resource="http://purl.obolibrary.org/obo/ENVO_00000004"/>
        <obo:RO_0001025 rdf:resource="http://purl.obolibrary.org/obo/GAZ_00010654"/>
        <obo:IAO_0000115>A district located in the southern part of Balkh Province, Afghanistan.</obo:IAO_0000115>
        <oboInOwl:hasOBONamespace>GAZ</oboInOwl:hasOBONamespace>
        <oboInOwl:id>GAZ:00021525</oboInOwl:id>
        <rdfs:label>Sholgara District</rdfs:label>
    </owl:NamedIndividual>
    


    <!-- http://purl.obolibrary.org/obo/GAZ_00021526 -->

    <owl:NamedIndividual rdf:about="http://purl.obolibrary.org/obo/GAZ_00021526">
        <rdf:type rdf:resource="http://purl.obolibrary.org/obo/ENVO_00000004"/>
        <obo:RO_0001025 rdf:resource="http://purl.obolibrary.org/obo/GAZ_00010654"/>
        <obo:IAO_0000115>A district of Balkh Province in Afghanistan.</obo:IAO_0000115>
        <oboInOwl:hasOBONamespace>GAZ</oboInOwl:hasOBONamespace>
        <oboInOwl:id>GAZ:00021526</oboInOwl:id>
        <rdfs:label>Khulm District</rdfs:label>
    </owl:NamedIndividual>
    


    <!-- http://purl.obolibrary.org/obo/GAZ_00021527 -->

    <owl:NamedIndividual rdf:about="http://purl.obolibrary.org/obo/GAZ_00021527">
        <rdf:type rdf:resource="http://purl.obolibrary.org/obo/ENVO_00000004"/>
        <obo:RO_0001025 rdf:resource="http://purl.obolibrary.org/obo/GAZ_00010657"/>
        <obo:IAO_0000115>A district located in the western end of the Bamyan Province in Afghanistan.</obo:IAO_0000115>
        <oboInOwl:hasOBONamespace>GAZ</oboInOwl:hasOBONamespace>
        <oboInOwl:id>GAZ:00021527</oboInOwl:id>
        <rdfs:label>Shibar District</rdfs:label>
    </owl:NamedIndividual>
    


    <!-- http://purl.obolibrary.org/obo/GAZ_00021528 -->

    <owl:NamedIndividual rdf:about="http://purl.obolibrary.org/obo/GAZ_00021528">
        <obo:RO_0001025 rdf:resource="http://purl.obolibrary.org/obo/GAZ_00010657"/>
        <obo:IAO_0000115>A mountainous district in the southern part of the Bamyan Province in Afghanistan.</obo:IAO_0000115>
        <oboInOwl:hasOBONamespace>GAZ</oboInOwl:hasOBONamespace>
        <oboInOwl:id>GAZ:00021528</oboInOwl:id>
        <rdfs:label>Waras District</rdfs:label>
    </owl:NamedIndividual>
    


    <!-- http://purl.obolibrary.org/obo/GAZ_00021529 -->

    <owl:NamedIndividual rdf:about="http://purl.obolibrary.org/obo/GAZ_00021529">
        <rdf:type rdf:resource="http://purl.obolibrary.org/obo/ENVO_00000004"/>
        <obo:RO_0001025 rdf:resource="http://purl.obolibrary.org/obo/GAZ_00010657"/>
        <obo:IAO_0000115>A district located in the northwestern part of Bamiyan Province.</obo:IAO_0000115>
        <oboInOwl:hasOBONamespace>GAZ</oboInOwl:hasOBONamespace>
        <oboInOwl:id>GAZ:00021529</oboInOwl:id>
        <rdfs:label>Yakawlang District</rdfs:label>
    </owl:NamedIndividual>
    


    <!-- http://purl.obolibrary.org/obo/GAZ_00021530 -->

    <owl:NamedIndividual rdf:about="http://purl.obolibrary.org/obo/GAZ_00021530">
        <rdf:type rdf:resource="http://purl.obolibrary.org/obo/ENVO_00000004"/>
        <obo:RO_0001025 rdf:resource="http://purl.obolibrary.org/obo/GAZ_00010657"/>
        <obo:IAO_0000115>A district in the central part of the Bamiyan Province.</obo:IAO_0000115>
        <oboInOwl:hasOBONamespace>GAZ</oboInOwl:hasOBONamespace>
        <oboInOwl:id>GAZ:00021530</oboInOwl:id>
        <rdfs:label>Panjab District</rdfs:label>
    </owl:NamedIndividual>
    


    <!-- http://purl.obolibrary.org/obo/GAZ_00021531 -->

    <owl:NamedIndividual rdf:about="http://purl.obolibrary.org/obo/GAZ_00021531">
        <obo:RO_0001025 rdf:resource="http://purl.obolibrary.org/obo/GAZ_00010657"/>
        <obo:IAO_0000115>The capital district in Bamyan Province, Afghanistan.</obo:IAO_0000115>
        <oboInOwl:hasOBONamespace>GAZ</oboInOwl:hasOBONamespace>
        <oboInOwl:id>GAZ:00021531</oboInOwl:id>
        <rdfs:label>Bayman District</rdfs:label>
    </owl:NamedIndividual>
    


    <!-- http://purl.obolibrary.org/obo/GAZ_00021532 -->

    <owl:NamedIndividual rdf:about="http://purl.obolibrary.org/obo/GAZ_00021532">
        <rdf:type rdf:resource="http://purl.obolibrary.org/obo/ENVO_00000004"/>
        <obo:RO_0001025 rdf:resource="http://purl.obolibrary.org/obo/GAZ_00010656"/>
        <obo:IAO_0000115>A district in Daykundi Province, Afghanistan.</obo:IAO_0000115>
        <oboInOwl:hasOBONamespace>GAZ</oboInOwl:hasOBONamespace>
        <oboInOwl:id>GAZ:00021532</oboInOwl:id>
        <rdfs:label>Day Kundi District</rdfs:label>
    </owl:NamedIndividual>
    


    <!-- http://purl.obolibrary.org/obo/GAZ_00021533 -->

    <owl:NamedIndividual rdf:about="http://purl.obolibrary.org/obo/GAZ_00021533">
        <rdf:type rdf:resource="http://purl.obolibrary.org/obo/ENVO_00000004"/>
        <obo:RO_0001025 rdf:resource="http://purl.obolibrary.org/obo/GAZ_00010629"/>
        <obo:IAO_0000115>A district in Oruzgan Province, Afghanistan. It had been in Daykundi Province but was re-annexed by Oruzgan Province in 2006.</obo:IAO_0000115>
        <oboInOwl:hasOBONamespace>GAZ</oboInOwl:hasOBONamespace>
        <oboInOwl:id>GAZ:00021533</oboInOwl:id>
        <rdfs:label>Gizab District</rdfs:label>
    </owl:NamedIndividual>
    


    <!-- http://purl.obolibrary.org/obo/GAZ_00021534 -->

    <owl:NamedIndividual rdf:about="http://purl.obolibrary.org/obo/GAZ_00021534">
        <rdf:type rdf:resource="http://purl.obolibrary.org/obo/ENVO_00000004"/>
        <obo:RO_0001025 rdf:resource="http://purl.obolibrary.org/obo/GAZ_00010656"/>
        <obo:IAO_0000115>A district in Daykundi Province, Afghanistan. It was transferred in 2004 from Uruzgan province.</obo:IAO_0000115>
        <oboInOwl:hasOBONamespace>GAZ</oboInOwl:hasOBONamespace>
        <oboInOwl:id>GAZ:00021534</oboInOwl:id>
        <rdfs:label>Shahristan District</rdfs:label>
    </owl:NamedIndividual>
    


    <!-- http://purl.obolibrary.org/obo/GAZ_00021535 -->

    <owl:NamedIndividual rdf:about="http://purl.obolibrary.org/obo/GAZ_00021535">
        <rdf:type rdf:resource="http://purl.obolibrary.org/obo/ENVO_00000004"/>
        <obo:RO_0001025 rdf:resource="http://purl.obolibrary.org/obo/GAZ_00010656"/>
        <obo:IAO_0000115>A district in Daykundi Province, Afghanistan. It was transferred in 2004 from Uruzgan province.</obo:IAO_0000115>
        <oboInOwl:hasOBONamespace>GAZ</oboInOwl:hasOBONamespace>
        <oboInOwl:id>GAZ:00021535</oboInOwl:id>
        <rdfs:label>Kijran District</rdfs:label>
    </owl:NamedIndividual>
    


    <!-- http://purl.obolibrary.org/obo/GAZ_00021536 -->

    <owl:NamedIndividual rdf:about="http://purl.obolibrary.org/obo/GAZ_00021536">
        <rdf:type rdf:resource="http://purl.obolibrary.org/obo/ENVO_00000004"/>
        <obo:RO_0001025 rdf:resource="http://purl.obolibrary.org/obo/GAZ_00010655"/>
        <obo:IAO_0000115>A district in Farah Province, Afghanistan.</obo:IAO_0000115>
        <oboInOwl:hasOBONamespace>GAZ</oboInOwl:hasOBONamespace>
        <oboInOwl:id>GAZ:00021536</oboInOwl:id>
        <rdfs:label>Bakwa District</rdfs:label>
    </owl:NamedIndividual>
    


    <!-- http://purl.obolibrary.org/obo/GAZ_00021537 -->

    <owl:NamedIndividual rdf:about="http://purl.obolibrary.org/obo/GAZ_00021537">
        <rdf:type rdf:resource="http://purl.obolibrary.org/obo/ENVO_00000004"/>
        <obo:RO_0001025 rdf:resource="http://purl.obolibrary.org/obo/GAZ_00010648"/>
        <obo:IAO_0000115>A district in the southern part of Faryab Province, Afghanistan.</obo:IAO_0000115>
        <oboInOwl:hasOBONamespace>GAZ</oboInOwl:hasOBONamespace>
        <oboInOwl:id>GAZ:00021537</oboInOwl:id>
        <rdfs:label>Bilchiragh District</rdfs:label>
    </owl:NamedIndividual>
    


    <!-- http://purl.obolibrary.org/obo/GAZ_00021538 -->

    <owl:NamedIndividual rdf:about="http://purl.obolibrary.org/obo/GAZ_00021538">
        <rdf:type rdf:resource="http://purl.obolibrary.org/obo/ENVO_00000004"/>
        <obo:RO_0001025 rdf:resource="http://purl.obolibrary.org/obo/GAZ_00010655"/>
        <obo:IAO_0000115>A district in Farah Province, Afghanistan.</obo:IAO_0000115>
        <oboInOwl:hasOBONamespace>GAZ</oboInOwl:hasOBONamespace>
        <oboInOwl:id>GAZ:00021538</oboInOwl:id>
        <rdfs:label>Shib Koh District</rdfs:label>
    </owl:NamedIndividual>
    


    <!-- http://purl.obolibrary.org/obo/GAZ_00021539 -->

    <owl:NamedIndividual rdf:about="http://purl.obolibrary.org/obo/GAZ_00021539">
        <rdf:type rdf:resource="http://purl.obolibrary.org/obo/ENVO_00000004"/>
        <obo:RO_0001025 rdf:resource="http://purl.obolibrary.org/obo/GAZ_00010655"/>
        <obo:IAO_0000115>A district in Farah Province, Afghanistan.</obo:IAO_0000115>
        <oboInOwl:hasOBONamespace>GAZ</oboInOwl:hasOBONamespace>
        <oboInOwl:id>GAZ:00021539</oboInOwl:id>
        <rdfs:label>Lash Wa Juwayn District</rdfs:label>
    </owl:NamedIndividual>
    


    <!-- http://purl.obolibrary.org/obo/GAZ_00021540 -->

    <owl:NamedIndividual rdf:about="http://purl.obolibrary.org/obo/GAZ_00021540">
        <rdf:type rdf:resource="http://purl.obolibrary.org/obo/ENVO_00000004"/>
        <obo:RO_0001025 rdf:resource="http://purl.obolibrary.org/obo/GAZ_00010655"/>
        <obo:IAO_0000115>A district in Farah Province, Afghanistan.</obo:IAO_0000115>
        <oboInOwl:hasOBONamespace>GAZ</oboInOwl:hasOBONamespace>
        <oboInOwl:id>GAZ:00021540</oboInOwl:id>
        <rdfs:label>Gulistan District</rdfs:label>
    </owl:NamedIndividual>
    


    <!-- http://purl.obolibrary.org/obo/GAZ_00021541 -->

    <owl:NamedIndividual rdf:about="http://purl.obolibrary.org/obo/GAZ_00021541">
        <rdf:type rdf:resource="http://purl.obolibrary.org/obo/ENVO_00000004"/>
        <obo:RO_0001025 rdf:resource="http://purl.obolibrary.org/obo/GAZ_00010655"/>
        <obo:IAO_0000115>A district in Farah Province, Afghanistan.</obo:IAO_0000115>
        <oboInOwl:hasOBONamespace>GAZ</oboInOwl:hasOBONamespace>
        <oboInOwl:id>GAZ:00021541</oboInOwl:id>
        <rdfs:label>Anar Dara District</rdfs:label>
    </owl:NamedIndividual>
    


    <!-- http://purl.obolibrary.org/obo/GAZ_00021542 -->

    <owl:NamedIndividual rdf:about="http://purl.obolibrary.org/obo/GAZ_00021542">
        <rdf:type rdf:resource="http://purl.obolibrary.org/obo/ENVO_00000004"/>
        <obo:RO_0001025 rdf:resource="http://purl.obolibrary.org/obo/GAZ_00010655"/>
        <obo:IAO_0000115>A district in Farah Province, Afghanistan.</obo:IAO_0000115>
        <oboInOwl:hasOBONamespace>GAZ</oboInOwl:hasOBONamespace>
        <oboInOwl:id>GAZ:00021542</oboInOwl:id>
        <rdfs:label>Pusht Rod District</rdfs:label>
    </owl:NamedIndividual>
    


    <!-- http://purl.obolibrary.org/obo/GAZ_00021543 -->

    <owl:NamedIndividual rdf:about="http://purl.obolibrary.org/obo/GAZ_00021543">
        <rdf:type rdf:resource="http://purl.obolibrary.org/obo/ENVO_00000004"/>
        <obo:RO_0001025 rdf:resource="http://purl.obolibrary.org/obo/GAZ_00010655"/>
        <obo:IAO_0000115>A district in Farah Province, Afghanistan.</obo:IAO_0000115>
        <oboInOwl:hasOBONamespace>GAZ</oboInOwl:hasOBONamespace>
        <oboInOwl:id>GAZ:00021543</oboInOwl:id>
        <rdfs:label>Bala Buluk District</rdfs:label>
    </owl:NamedIndividual>
    


    <!-- http://purl.obolibrary.org/obo/GAZ_00021544 -->

    <owl:NamedIndividual rdf:about="http://purl.obolibrary.org/obo/GAZ_00021544">
        <rdf:type rdf:resource="http://purl.obolibrary.org/obo/ENVO_00000004"/>
        <obo:RO_0001025 rdf:resource="http://purl.obolibrary.org/obo/GAZ_00010655"/>
        <obo:IAO_0000115>A district in Farah Province, Afghanistan.</obo:IAO_0000115>
        <oboInOwl:hasOBONamespace>GAZ</oboInOwl:hasOBONamespace>
        <oboInOwl:id>GAZ:00021544</oboInOwl:id>
        <rdfs:label>Khaki Safed District</rdfs:label>
    </owl:NamedIndividual>
    


    <!-- http://purl.obolibrary.org/obo/GAZ_00021545 -->

    <owl:NamedIndividual rdf:about="http://purl.obolibrary.org/obo/GAZ_00021545">
        <rdf:type rdf:resource="http://purl.obolibrary.org/obo/ENVO_00000004"/>
        <obo:RO_0001025 rdf:resource="http://purl.obolibrary.org/obo/GAZ_00010655"/>
        <obo:IAO_0000115>A district in Farah Province, Afghanistan, containing the main city of Farah.</obo:IAO_0000115>
        <oboInOwl:hasOBONamespace>GAZ</oboInOwl:hasOBONamespace>
        <oboInOwl:id>GAZ:00021545</oboInOwl:id>
        <rdfs:label>Farah District</rdfs:label>
    </owl:NamedIndividual>
    


    <!-- http://purl.obolibrary.org/obo/GAZ_00021546 -->

    <owl:NamedIndividual rdf:about="http://purl.obolibrary.org/obo/GAZ_00021546">
        <obo:RO_0001025 rdf:resource="http://purl.obolibrary.org/obo/GAZ_00010655"/>
        <obo:IAO_0000115>A mountainous district in Farah Province, Afghanistan.</obo:IAO_0000115>
        <oboInOwl:hasOBONamespace>GAZ</oboInOwl:hasOBONamespace>
        <oboInOwl:id>GAZ:00021546</oboInOwl:id>
        <rdfs:label>Pur Chaman District</rdfs:label>
    </owl:NamedIndividual>
    


    <!-- http://purl.obolibrary.org/obo/GAZ_00021547 -->

    <owl:NamedIndividual rdf:about="http://purl.obolibrary.org/obo/GAZ_00021547">
        <rdf:type rdf:resource="http://purl.obolibrary.org/obo/ENVO_00000004"/>
        <obo:RO_0001025 rdf:resource="http://purl.obolibrary.org/obo/GAZ_00010655"/>
        <obo:IAO_0000115>A district located in the western part of the Farah Province. Its western border is with Iran.</obo:IAO_0000115>
        <oboInOwl:hasOBONamespace>GAZ</oboInOwl:hasOBONamespace>
        <oboInOwl:id>GAZ:00021547</oboInOwl:id>
        <rdfs:label>Qala-I-Kah District</rdfs:label>
    </owl:NamedIndividual>
    


    <!-- http://purl.obolibrary.org/obo/GAZ_00021548 -->

    <owl:NamedIndividual rdf:about="http://purl.obolibrary.org/obo/GAZ_00021548">
        <rdf:type rdf:resource="http://purl.obolibrary.org/obo/ENVO_00000004"/>
        <obo:RO_0001025 rdf:resource="http://purl.obolibrary.org/obo/GAZ_00010648"/>
        <obo:IAO_0000115>A district in Faryab Province, Afghanistan.</obo:IAO_0000115>
        <oboInOwl:hasOBONamespace>GAZ</oboInOwl:hasOBONamespace>
        <oboInOwl:id>GAZ:00021548</oboInOwl:id>
        <rdfs:label>Dawlatabad District</rdfs:label>
    </owl:NamedIndividual>
    


    <!-- http://purl.obolibrary.org/obo/GAZ_00021549 -->

    <owl:NamedIndividual rdf:about="http://purl.obolibrary.org/obo/GAZ_00021549">
        <rdf:type rdf:resource="http://purl.obolibrary.org/obo/ENVO_00000004"/>
        <obo:RO_0001025 rdf:resource="http://purl.obolibrary.org/obo/GAZ_00010648"/>
        <obo:IAO_0000115>A district located south of Andkhoy in the northern part of Faryab Province.</obo:IAO_0000115>
        <oboInOwl:hasOBONamespace>GAZ</oboInOwl:hasOBONamespace>
        <oboInOwl:id>GAZ:00021549</oboInOwl:id>
        <rdfs:label>Qaramqol District</rdfs:label>
    </owl:NamedIndividual>
    


    <!-- http://purl.obolibrary.org/obo/GAZ_00021550 -->

    <owl:NamedIndividual rdf:about="http://purl.obolibrary.org/obo/GAZ_00021550">
        <obo:RO_0001025 rdf:resource="http://purl.obolibrary.org/obo/GAZ_00010648"/>
        <obo:IAO_0000115>A district is located in the center of Faryab Province southeast from Maymana.</obo:IAO_0000115>
        <oboInOwl:hasOBONamespace>GAZ</oboInOwl:hasOBONamespace>
        <oboInOwl:id>GAZ:00021550</oboInOwl:id>
        <rdfs:label>Pushtun Kot District</rdfs:label>
    </owl:NamedIndividual>
    


    <!-- http://purl.obolibrary.org/obo/GAZ_00021551 -->

    <owl:NamedIndividual rdf:about="http://purl.obolibrary.org/obo/GAZ_00021551">
        <rdf:type rdf:resource="http://purl.obolibrary.org/obo/ENVO_00000004"/>
        <obo:RO_0001025 rdf:resource="http://purl.obolibrary.org/obo/GAZ_00010648"/>
        <obo:IAO_0000115>A district in Faryab Province, Afghanistan.</obo:IAO_0000115>
        <oboInOwl:hasOBONamespace>GAZ</oboInOwl:hasOBONamespace>
        <oboInOwl:id>GAZ:00021551</oboInOwl:id>
        <rdfs:label>Shirin Tagab District</rdfs:label>
    </owl:NamedIndividual>
    


    <!-- http://purl.obolibrary.org/obo/GAZ_00021552 -->

    <owl:NamedIndividual rdf:about="http://purl.obolibrary.org/obo/GAZ_00021552">
        <obo:RO_0001025 rdf:resource="http://purl.obolibrary.org/obo/GAZ_00010648"/>
        <obo:IAO_0000115>The most northerly district in Faryab Province.</obo:IAO_0000115>
        <oboInOwl:hasOBONamespace>GAZ</oboInOwl:hasOBONamespace>
        <oboInOwl:id>GAZ:00021552</oboInOwl:id>
        <rdfs:label>Khani Chahar Bagh District</rdfs:label>
    </owl:NamedIndividual>
    


    <!-- http://purl.obolibrary.org/obo/GAZ_00021553 -->

    <owl:NamedIndividual rdf:about="http://purl.obolibrary.org/obo/GAZ_00021553">
        <rdf:type rdf:resource="http://purl.obolibrary.org/obo/ENVO_00000004"/>
        <obo:RO_0001025 rdf:resource="http://purl.obolibrary.org/obo/GAZ_00010648"/>
        <obo:IAO_0000115>A district in Faryab Province, Afghanistan.</obo:IAO_0000115>
        <oboInOwl:hasOBONamespace>GAZ</oboInOwl:hasOBONamespace>
        <oboInOwl:id>GAZ:00021553</oboInOwl:id>
        <rdfs:label>Khwaja Sabz District</rdfs:label>
    </owl:NamedIndividual>
    


    <!-- http://purl.obolibrary.org/obo/GAZ_00021554 -->

    <owl:NamedIndividual rdf:about="http://purl.obolibrary.org/obo/GAZ_00021554">
        <rdf:type rdf:resource="http://purl.obolibrary.org/obo/ENVO_00000004"/>
        <obo:RO_0001025 rdf:resource="http://purl.obolibrary.org/obo/GAZ_00010648"/>
        <obo:IAO_0000115>A district located in the southwestern part of Faryab Province.</obo:IAO_0000115>
        <oboInOwl:hasOBONamespace>GAZ</oboInOwl:hasOBONamespace>
        <oboInOwl:id>GAZ:00021554</oboInOwl:id>
        <rdfs:label>Qaysar District</rdfs:label>
    </owl:NamedIndividual>
    


    <!-- http://purl.obolibrary.org/obo/GAZ_00021555 -->

    <owl:NamedIndividual rdf:about="http://purl.obolibrary.org/obo/GAZ_00021555">
        <obo:RO_0001025 rdf:resource="http://purl.obolibrary.org/obo/GAZ_00010648"/>
        <obo:IAO_0000115>The capital district of Faryab province, northern Afghanistan, near the Uzbekistan border.</obo:IAO_0000115>
        <oboInOwl:hasOBONamespace>GAZ</oboInOwl:hasOBONamespace>
        <oboInOwl:id>GAZ:00021555</oboInOwl:id>
        <rdfs:label>Maymana District</rdfs:label>
    </owl:NamedIndividual>
    


    <!-- http://purl.obolibrary.org/obo/GAZ_00021556 -->

    <owl:NamedIndividual rdf:about="http://purl.obolibrary.org/obo/GAZ_00021556">
        <obo:RO_0001025 rdf:resource="http://purl.obolibrary.org/obo/GAZ_00010648"/>
        <obo:IAO_0000115>The southern-most district in Faryab Province.</obo:IAO_0000115>
        <oboInOwl:hasOBONamespace>GAZ</oboInOwl:hasOBONamespace>
        <oboInOwl:id>GAZ:00021556</oboInOwl:id>
        <rdfs:label>Kohistan District</rdfs:label>
    </owl:NamedIndividual>
    


    <!-- http://purl.obolibrary.org/obo/GAZ_00021557 -->

    <owl:NamedIndividual rdf:about="http://purl.obolibrary.org/obo/GAZ_00021557">
        <rdf:type rdf:resource="http://purl.obolibrary.org/obo/ENVO_00000004"/>
        <obo:RO_0001025 rdf:resource="http://purl.obolibrary.org/obo/GAZ_00010648"/>
        <obo:IAO_0000115>A district in the southwestern part of Faryab Province, Afghanistan. Its northern border is the national border with Turkmenistan.</obo:IAO_0000115>
        <oboInOwl:hasOBONamespace>GAZ</oboInOwl:hasOBONamespace>
        <oboInOwl:id>GAZ:00021557</oboInOwl:id>
        <rdfs:label>Almar District</rdfs:label>
    </owl:NamedIndividual>
    


    <!-- http://purl.obolibrary.org/obo/GAZ_00021558 -->

    <owl:NamedIndividual rdf:about="http://purl.obolibrary.org/obo/GAZ_00021558">
        <rdf:type rdf:resource="http://purl.obolibrary.org/obo/ENVO_00000004"/>
        <obo:RO_0001025 rdf:resource="http://purl.obolibrary.org/obo/GAZ_00010648"/>
        <obo:IAO_0000115>A district in northern Afghanistan, Faryab Province.</obo:IAO_0000115>
        <oboInOwl:hasOBONamespace>GAZ</oboInOwl:hasOBONamespace>
        <oboInOwl:id>GAZ:00021558</oboInOwl:id>
        <rdfs:label>Andkhoy District</rdfs:label>
    </owl:NamedIndividual>
    


    <!-- http://purl.obolibrary.org/obo/GAZ_00021559 -->

    <owl:NamedIndividual rdf:about="http://purl.obolibrary.org/obo/GAZ_00021559">
        <rdf:type rdf:resource="http://purl.obolibrary.org/obo/ENVO_00000004"/>
        <obo:RO_0001025 rdf:resource="http://purl.obolibrary.org/obo/GAZ_00010652"/>
        <obo:IAO_0000115>A district in the south of Ghazni Province, Afghanistan.</obo:IAO_0000115>
        <oboInOwl:hasOBONamespace>GAZ</oboInOwl:hasOBONamespace>
        <oboInOwl:id>GAZ:00021559</oboInOwl:id>
        <rdfs:label>Gelan District</rdfs:label>
    </owl:NamedIndividual>
    


    <!-- http://purl.obolibrary.org/obo/GAZ_00021560 -->

    <owl:NamedIndividual rdf:about="http://purl.obolibrary.org/obo/GAZ_00021560">
        <obo:RO_0001025 rdf:resource="http://purl.obolibrary.org/obo/GAZ_00010652"/>
        <obo:IAO_0000115>A mountainous district in Ghazni Province, Afghanistan.</obo:IAO_0000115>
        <oboInOwl:hasOBONamespace>GAZ</oboInOwl:hasOBONamespace>
        <oboInOwl:id>GAZ:00021560</oboInOwl:id>
        <rdfs:label>Zana Khan District</rdfs:label>
    </owl:NamedIndividual>
    


    <!-- http://purl.obolibrary.org/obo/GAZ_00021561 -->

    <owl:NamedIndividual rdf:about="http://purl.obolibrary.org/obo/GAZ_00021561">
        <obo:RO_0001025 rdf:resource="http://purl.obolibrary.org/obo/GAZ_00010652"/>
        <obo:IAO_0000115>One of the eastern districts of Ghazni Province in Afghanistan.</obo:IAO_0000115>
        <oboInOwl:hasOBONamespace>GAZ</oboInOwl:hasOBONamespace>
        <oboInOwl:id>GAZ:00021561</oboInOwl:id>
        <rdfs:label>Andar District</rdfs:label>
    </owl:NamedIndividual>
    


    <!-- http://purl.obolibrary.org/obo/GAZ_00021562 -->

    <owl:NamedIndividual rdf:about="http://purl.obolibrary.org/obo/GAZ_00021562">
        <obo:RO_0001025 rdf:resource="http://purl.obolibrary.org/obo/GAZ_00010652"/>
        <oboInOwl:hasOBONamespace>GAZ</oboInOwl:hasOBONamespace>
        <oboInOwl:id>GAZ:00021562</oboInOwl:id>
        <rdfs:label>[Former] Bahrami Shahid District</rdfs:label>
    </owl:NamedIndividual>
    


    <!-- http://purl.obolibrary.org/obo/GAZ_00021563 -->

    <owl:NamedIndividual rdf:about="http://purl.obolibrary.org/obo/GAZ_00021563">
        <rdf:type rdf:resource="http://purl.obolibrary.org/obo/ENVO_00000004"/>
        <obo:RO_0001025 rdf:resource="http://purl.obolibrary.org/obo/GAZ_00010640"/>
        <obo:IAO_0000115>A district in Wardak Province, Afghanistan, 40 km northwest of Ghazni.</obo:IAO_0000115>
        <oboInOwl:hasOBONamespace>GAZ</oboInOwl:hasOBONamespace>
        <oboInOwl:id>GAZ:00021563</oboInOwl:id>
        <rdfs:label>Jaghatu District</rdfs:label>
    </owl:NamedIndividual>
    


    <!-- http://purl.obolibrary.org/obo/GAZ_00021564 -->

    <owl:NamedIndividual rdf:about="http://purl.obolibrary.org/obo/GAZ_00021564">
        <rdf:type rdf:resource="http://purl.obolibrary.org/obo/ENVO_00000004"/>
        <obo:RO_0001025 rdf:resource="http://purl.obolibrary.org/obo/GAZ_00010649"/>
        <obo:IAO_0000115>A district located in the southern part of Ghor Province, Afghanistan.</obo:IAO_0000115>
        <oboInOwl:hasOBONamespace>GAZ</oboInOwl:hasOBONamespace>
        <oboInOwl:id>GAZ:00021564</oboInOwl:id>
        <rdfs:label>Pasaband District</rdfs:label>
    </owl:NamedIndividual>
    


    <!-- http://purl.obolibrary.org/obo/GAZ_00021565 -->

    <owl:NamedIndividual rdf:about="http://purl.obolibrary.org/obo/GAZ_00021565">
        <rdf:type rdf:resource="http://purl.obolibrary.org/obo/ENVO_00000004"/>
        <obo:RO_0001025 rdf:resource="http://purl.obolibrary.org/obo/GAZ_00010652"/>
        <obo:IAO_0000115>A district in Ghazni Province, Afghanistan.</obo:IAO_0000115>
        <oboInOwl:hasOBONamespace>GAZ</oboInOwl:hasOBONamespace>
        <oboInOwl:id>GAZ:00021565</oboInOwl:id>
        <rdfs:label>Jaghuri District</rdfs:label>
    </owl:NamedIndividual>
    


    <!-- http://purl.obolibrary.org/obo/GAZ_00021566 -->

    <owl:NamedIndividual rdf:about="http://purl.obolibrary.org/obo/GAZ_00021566">
        <rdf:type rdf:resource="http://purl.obolibrary.org/obo/ENVO_00000004"/>
        <obo:RO_0001025 rdf:resource="http://purl.obolibrary.org/obo/GAZ_00010652"/>
        <obo:IAO_0000115>A district in Ghazni Province, Afghanistan.</obo:IAO_0000115>
        <oboInOwl:hasOBONamespace>GAZ</oboInOwl:hasOBONamespace>
        <oboInOwl:id>GAZ:00021566</oboInOwl:id>
        <rdfs:label>Ab Band District</rdfs:label>
    </owl:NamedIndividual>
    


    <!-- http://purl.obolibrary.org/obo/GAZ_00021567 -->

    <owl:NamedIndividual rdf:about="http://purl.obolibrary.org/obo/GAZ_00021567">
        <rdf:type rdf:resource="http://purl.obolibrary.org/obo/ENVO_00000004"/>
        <obo:RO_0001025 rdf:resource="http://purl.obolibrary.org/obo/GAZ_00010652"/>
        <obo:IAO_0000115>A district in the eastern part of Ghazni Province.</obo:IAO_0000115>
        <oboInOwl:hasOBONamespace>GAZ</oboInOwl:hasOBONamespace>
        <oboInOwl:id>GAZ:00021567</oboInOwl:id>
        <rdfs:label>Dih Yak District</rdfs:label>
    </owl:NamedIndividual>
    


    <!-- http://purl.obolibrary.org/obo/GAZ_00021568 -->

    <owl:NamedIndividual rdf:about="http://purl.obolibrary.org/obo/GAZ_00021568">
        <obo:RO_0001025 rdf:resource="http://purl.obolibrary.org/obo/GAZ_00010652"/>
        <obo:IAO_0000115>The capital district of Ghazni Province, Afghanistan.</obo:IAO_0000115>
        <oboInOwl:hasOBONamespace>GAZ</oboInOwl:hasOBONamespace>
        <oboInOwl:id>GAZ:00021568</oboInOwl:id>
        <rdfs:label>Ghazni District</rdfs:label>
    </owl:NamedIndividual>
    


    <!-- http://purl.obolibrary.org/obo/GAZ_00021569 -->

    <owl:NamedIndividual rdf:about="http://purl.obolibrary.org/obo/GAZ_00021569">
        <rdf:type rdf:resource="http://purl.obolibrary.org/obo/ENVO_00000004"/>
        <obo:RO_0001025 rdf:resource="http://purl.obolibrary.org/obo/GAZ_00010652"/>
        <obo:IAO_0000115>A large district in the far south of Ghazni Province, Afghanistan.</obo:IAO_0000115>
        <oboInOwl:hasOBONamespace>GAZ</oboInOwl:hasOBONamespace>
        <oboInOwl:id>GAZ:00021569</oboInOwl:id>
        <rdfs:label>Nawa District</rdfs:label>
    </owl:NamedIndividual>
    


    <!-- http://purl.obolibrary.org/obo/GAZ_00021570 -->

    <owl:NamedIndividual rdf:about="http://purl.obolibrary.org/obo/GAZ_00021570">
        <rdf:type rdf:resource="http://purl.obolibrary.org/obo/ENVO_00000004"/>
        <obo:RO_0001025 rdf:resource="http://purl.obolibrary.org/obo/GAZ_00010652"/>
        <obo:IAO_0000115>A district in the west of Ghazni Province, Afghanistan.</obo:IAO_0000115>
        <oboInOwl:hasOBONamespace>GAZ</oboInOwl:hasOBONamespace>
        <oboInOwl:id>GAZ:00021570</oboInOwl:id>
        <rdfs:label>Ajristan District</rdfs:label>
    </owl:NamedIndividual>
    


    <!-- http://purl.obolibrary.org/obo/GAZ_00021571 -->

    <owl:NamedIndividual rdf:about="http://purl.obolibrary.org/obo/GAZ_00021571">
        <obo:RO_0001025 rdf:resource="http://purl.obolibrary.org/obo/GAZ_00010652"/>
        <obo:IAO_0000115>The largest district in Ghazni Province, Afghanistan.</obo:IAO_0000115>
        <oboInOwl:hasOBONamespace>GAZ</oboInOwl:hasOBONamespace>
        <oboInOwl:id>GAZ:00021571</oboInOwl:id>
        <rdfs:label>Nawur District</rdfs:label>
    </owl:NamedIndividual>
    


    <!-- http://purl.obolibrary.org/obo/GAZ_00021572 -->

    <owl:NamedIndividual rdf:about="http://purl.obolibrary.org/obo/GAZ_00021572">
        <rdf:type rdf:resource="http://purl.obolibrary.org/obo/ENVO_00000004"/>
        <obo:RO_0001025 rdf:resource="http://purl.obolibrary.org/obo/GAZ_00010652"/>
        <obo:IAO_0000115>A district in the southwest of Ghazni Province, Afghanistan.</obo:IAO_0000115>
        <oboInOwl:hasOBONamespace>GAZ</oboInOwl:hasOBONamespace>
        <oboInOwl:id>GAZ:00021572</oboInOwl:id>
        <rdfs:label>Muqur District</rdfs:label>
    </owl:NamedIndividual>
    


    <!-- http://purl.obolibrary.org/obo/GAZ_00021573 -->

    <owl:NamedIndividual rdf:about="http://purl.obolibrary.org/obo/GAZ_00021573">
        <rdf:type rdf:resource="http://purl.obolibrary.org/obo/ENVO_00000004"/>
        <obo:RO_0001025 rdf:resource="http://purl.obolibrary.org/obo/GAZ_00010652"/>
        <obo:IAO_0000115>A district located 56 km to South West of Ghazni.</obo:IAO_0000115>
        <oboInOwl:hasOBONamespace>GAZ</oboInOwl:hasOBONamespace>
        <oboInOwl:id>GAZ:00021573</oboInOwl:id>
        <rdfs:label>Qarabagh District</rdfs:label>
    </owl:NamedIndividual>
    


    <!-- http://purl.obolibrary.org/obo/GAZ_00021574 -->

    <owl:NamedIndividual rdf:about="http://purl.obolibrary.org/obo/GAZ_00021574">
        <rdf:type rdf:resource="http://purl.obolibrary.org/obo/ENVO_00000004"/>
        <obo:RO_0001025 rdf:resource="http://purl.obolibrary.org/obo/GAZ_00010652"/>
        <obo:IAO_0000115>A district located on the southeastern part of Ghazni Province in Afghanistan.</obo:IAO_0000115>
        <oboInOwl:hasOBONamespace>GAZ</oboInOwl:hasOBONamespace>
        <oboInOwl:id>GAZ:00021574</oboInOwl:id>
        <rdfs:label>Giro District</rdfs:label>
    </owl:NamedIndividual>
    


    <!-- http://purl.obolibrary.org/obo/GAZ_00021575 -->

    <owl:NamedIndividual rdf:about="http://purl.obolibrary.org/obo/GAZ_00021575">
        <rdf:type rdf:resource="http://purl.obolibrary.org/obo/ENVO_00000004"/>
        <obo:RO_0001025 rdf:resource="http://purl.obolibrary.org/obo/GAZ_00010652"/>
        <obo:IAO_0000115>A district in the west of Ghazni Province, Afghanistan.</obo:IAO_0000115>
        <oboInOwl:hasOBONamespace>GAZ</oboInOwl:hasOBONamespace>
        <oboInOwl:id>GAZ:00021575</oboInOwl:id>
        <rdfs:label>Malistan District</rdfs:label>
    </owl:NamedIndividual>
    


    <!-- http://purl.obolibrary.org/obo/GAZ_00021576 -->

    <owl:NamedIndividual rdf:about="http://purl.obolibrary.org/obo/GAZ_00021576">
        <rdf:type rdf:resource="http://purl.obolibrary.org/obo/ENVO_00000004"/>
        <obo:RO_0001025 rdf:resource="http://purl.obolibrary.org/obo/GAZ_00010649"/>
        <obo:IAO_0000115>A district located in the southern part of Ghor Province in Afghanistan.</obo:IAO_0000115>
        <oboInOwl:hasOBONamespace>GAZ</oboInOwl:hasOBONamespace>
        <oboInOwl:id>GAZ:00021576</oboInOwl:id>
        <rdfs:label>Taywara District</rdfs:label>
    </owl:NamedIndividual>
    


    <!-- http://purl.obolibrary.org/obo/GAZ_00021577 -->

    <owl:NamedIndividual rdf:about="http://purl.obolibrary.org/obo/GAZ_00021577">
        <obo:RO_0001025 rdf:resource="http://purl.obolibrary.org/obo/GAZ_00010649"/>
        <obo:IAO_0000115>The capital district of Ghor Province, Afghanistan.</obo:IAO_0000115>
        <oboInOwl:hasOBONamespace>GAZ</oboInOwl:hasOBONamespace>
        <oboInOwl:id>GAZ:00021577</oboInOwl:id>
        <rdfs:label>Chaghcharan District</rdfs:label>
    </owl:NamedIndividual>
    


    <!-- http://purl.obolibrary.org/obo/GAZ_00021578 -->

    <owl:NamedIndividual rdf:about="http://purl.obolibrary.org/obo/GAZ_00021578">
        <rdf:type rdf:resource="http://purl.obolibrary.org/obo/ENVO_00000004"/>
        <obo:RO_0001025 rdf:resource="http://purl.obolibrary.org/obo/GAZ_00010649"/>
        <obo:IAO_0000115>A district in the north of Ghor Province, Afghanistan.</obo:IAO_0000115>
        <oboInOwl:hasOBONamespace>GAZ</oboInOwl:hasOBONamespace>
        <oboInOwl:id>GAZ:00021578</oboInOwl:id>
        <rdfs:label>Lal Wa Sarjangal District</rdfs:label>
    </owl:NamedIndividual>
    


    <!-- http://purl.obolibrary.org/obo/GAZ_00021579 -->

    <owl:NamedIndividual rdf:about="http://purl.obolibrary.org/obo/GAZ_00021579">
        <rdf:type rdf:resource="http://purl.obolibrary.org/obo/ENVO_00000004"/>
        <obo:RO_0001025 rdf:resource="http://purl.obolibrary.org/obo/GAZ_00010649"/>
        <obo:IAO_0000115>A district located in the southwestern part of the Ghor Province, Afghanistan.</obo:IAO_0000115>
        <oboInOwl:hasOBONamespace>GAZ</oboInOwl:hasOBONamespace>
        <oboInOwl:id>GAZ:00021579</oboInOwl:id>
        <rdfs:label>Tulak District</rdfs:label>
    </owl:NamedIndividual>
    


    <!-- http://purl.obolibrary.org/obo/GAZ_00021580 -->

    <owl:NamedIndividual rdf:about="http://purl.obolibrary.org/obo/GAZ_00021580">
        <rdf:type rdf:resource="http://purl.obolibrary.org/obo/ENVO_00000004"/>
        <obo:RO_0001025 rdf:resource="http://purl.obolibrary.org/obo/GAZ_00010649"/>
        <obo:IAO_0000115>A district in the most southwestern part of Ghor Province, Afghanistan.</obo:IAO_0000115>
        <oboInOwl:hasOBONamespace>GAZ</oboInOwl:hasOBONamespace>
        <oboInOwl:id>GAZ:00021580</oboInOwl:id>
        <rdfs:label>Saghar District</rdfs:label>
    </owl:NamedIndividual>
    


    <!-- http://purl.obolibrary.org/obo/GAZ_00021581 -->

    <owl:NamedIndividual rdf:about="http://purl.obolibrary.org/obo/GAZ_00021581">
        <rdf:type rdf:resource="http://purl.obolibrary.org/obo/ENVO_00000004"/>
        <obo:RO_0001025 rdf:resource="http://purl.obolibrary.org/obo/GAZ_00010649"/>
        <obo:IAO_0000115>A district located in the central part of Ghor Province, Afghanistan.</obo:IAO_0000115>
        <oboInOwl:hasOBONamespace>GAZ</oboInOwl:hasOBONamespace>
        <oboInOwl:id>GAZ:00021581</oboInOwl:id>
        <rdfs:label>Shahrak District</rdfs:label>
    </owl:NamedIndividual>
    


    <!-- http://purl.obolibrary.org/obo/GAZ_00021582 -->

    <owl:NamedIndividual rdf:about="http://purl.obolibrary.org/obo/GAZ_00021582">
        <rdf:type rdf:resource="http://purl.obolibrary.org/obo/ENVO_00000004"/>
        <obo:RO_0001025 rdf:resource="http://purl.obolibrary.org/obo/GAZ_00010650"/>
        <obo:IAO_0000115>A district in the east of Helmand Province, Afghanistan.</obo:IAO_0000115>
        <oboInOwl:hasOBONamespace>GAZ</oboInOwl:hasOBONamespace>
        <oboInOwl:id>GAZ:00021582</oboInOwl:id>
        <rdfs:label>Kajaki District</rdfs:label>
    </owl:NamedIndividual>
    


    <!-- http://purl.obolibrary.org/obo/GAZ_00021583 -->

    <owl:NamedIndividual rdf:about="http://purl.obolibrary.org/obo/GAZ_00021583">
        <rdf:type rdf:resource="http://purl.obolibrary.org/obo/ENVO_00000004"/>
        <obo:RO_0001025 rdf:resource="http://purl.obolibrary.org/obo/GAZ_00010650"/>
        <obo:IAO_0000115>A district in the south of Helmand Province, Afghanistan, bordering on Pakistan.</obo:IAO_0000115>
        <oboInOwl:hasOBONamespace>GAZ</oboInOwl:hasOBONamespace>
        <oboInOwl:id>GAZ:00021583</oboInOwl:id>
        <rdfs:label>Dishu District</rdfs:label>
    </owl:NamedIndividual>
    


    <!-- http://purl.obolibrary.org/obo/GAZ_00021584 -->

    <owl:NamedIndividual rdf:about="http://purl.obolibrary.org/obo/GAZ_00021584">
        <rdf:type rdf:resource="http://purl.obolibrary.org/obo/ENVO_00000004"/>
        <obo:RO_0001025 rdf:resource="http://purl.obolibrary.org/obo/GAZ_00010650"/>
        <obo:IAO_0000115>A district in the west of Helmand Province, Afghanistan.</obo:IAO_0000115>
        <oboInOwl:hasOBONamespace>GAZ</oboInOwl:hasOBONamespace>
        <oboInOwl:id>GAZ:00021584</oboInOwl:id>
        <rdfs:label>Washer District</rdfs:label>
    </owl:NamedIndividual>
    


    <!-- http://purl.obolibrary.org/obo/GAZ_00021585 -->

    <owl:NamedIndividual rdf:about="http://purl.obolibrary.org/obo/GAZ_00021585">
        <rdf:type rdf:resource="http://purl.obolibrary.org/obo/ENVO_00000004"/>
        <obo:RO_0001025 rdf:resource="http://purl.obolibrary.org/obo/GAZ_00010650"/>
        <obo:IAO_0000115>A district in the north of Helmand Province, Afghanistan.</obo:IAO_0000115>
        <oboInOwl:hasOBONamespace>GAZ</oboInOwl:hasOBONamespace>
        <oboInOwl:id>GAZ:00021585</oboInOwl:id>
        <rdfs:label>Musa Qala District</rdfs:label>
    </owl:NamedIndividual>
    


    <!-- http://purl.obolibrary.org/obo/GAZ_00021586 -->

    <owl:NamedIndividual rdf:about="http://purl.obolibrary.org/obo/GAZ_00021586">
        <obo:RO_0001025 rdf:resource="http://purl.obolibrary.org/obo/GAZ_00010653"/>
        <obo:IAO_0000115>A district situated in the western part of Herat Province, Afghanistan. It borders on Iran to the west and northwest. To the north it borders on Kohsan District, to the east on Zendeh Jan District and to the south on Adraskan District. The Hari River flows through the northeastern end of the district.</obo:IAO_0000115>
        <oboInOwl:hasOBONamespace>GAZ</oboInOwl:hasOBONamespace>
        <oboInOwl:id>GAZ:00021586</oboInOwl:id>
        <rdfs:label>Ghoryan District</rdfs:label>
    </owl:NamedIndividual>
    


    <!-- http://purl.obolibrary.org/obo/GAZ_00021587 -->

    <owl:NamedIndividual rdf:about="http://purl.obolibrary.org/obo/GAZ_00021587">
        <rdf:type rdf:resource="http://purl.obolibrary.org/obo/ENVO_00000004"/>
        <obo:RO_0001025 rdf:resource="http://purl.obolibrary.org/obo/GAZ_00010650"/>
        <obo:IAO_0000115>A district in the east of Helmand Province, Afghanistan, surrounding the provincial capital of Lashkar Gah.</obo:IAO_0000115>
        <oboInOwl:hasOBONamespace>GAZ</oboInOwl:hasOBONamespace>
        <oboInOwl:id>GAZ:00021587</oboInOwl:id>
        <rdfs:label>Lashkar Gah District</rdfs:label>
    </owl:NamedIndividual>
    


    <!-- http://purl.obolibrary.org/obo/GAZ_00021588 -->

    <owl:NamedIndividual rdf:about="http://purl.obolibrary.org/obo/GAZ_00021588">
        <obo:RO_0001025 rdf:resource="http://purl.obolibrary.org/obo/GAZ_00010653"/>
        <obo:IAO_0000115>A district situated in the Northeastern part of the Herat Province in Afghanistan. It borders with Kushk District to the North-West, Kushki Kuhna District to the North and Badghis Province to the North-East. To the East is the Obe District. To the South is the Pashtun Zarghun District and the Injil District is situated to the West.</obo:IAO_0000115>
        <oboInOwl:hasOBONamespace>GAZ</oboInOwl:hasOBONamespace>
        <oboInOwl:id>GAZ:00021588</oboInOwl:id>
        <rdfs:label>Karukh District</rdfs:label>
    </owl:NamedIndividual>
    


    <!-- http://purl.obolibrary.org/obo/GAZ_00021589 -->

    <owl:NamedIndividual rdf:about="http://purl.obolibrary.org/obo/GAZ_00021589">
        <rdf:type rdf:resource="http://purl.obolibrary.org/obo/ENVO_00000004"/>
        <obo:RO_0001025 rdf:resource="http://purl.obolibrary.org/obo/GAZ_00010653"/>
        <obo:IAO_0000115>A district of Herat Province.</obo:IAO_0000115>
        <oboInOwl:hasOBONamespace>GAZ</oboInOwl:hasOBONamespace>
        <oboInOwl:id>GAZ:00021589</oboInOwl:id>
        <rdfs:label>Hirat District</rdfs:label>
    </owl:NamedIndividual>
    


    <!-- http://purl.obolibrary.org/obo/GAZ_00021590 -->

    <owl:NamedIndividual rdf:about="http://purl.obolibrary.org/obo/GAZ_00021590">
        <obo:RO_0001025 rdf:resource="http://purl.obolibrary.org/obo/GAZ_00010650"/>
        <obo:IAO_0000115>The northernmost district in Helmand Province, Afghanistan.</obo:IAO_0000115>
        <oboInOwl:hasOBONamespace>GAZ</oboInOwl:hasOBONamespace>
        <oboInOwl:id>GAZ:00021590</oboInOwl:id>
        <rdfs:label>Baghran District</rdfs:label>
    </owl:NamedIndividual>
    


    <!-- http://purl.obolibrary.org/obo/GAZ_00021592 -->

    <owl:NamedIndividual rdf:about="http://purl.obolibrary.org/obo/GAZ_00021592">
        <rdf:type rdf:resource="http://purl.obolibrary.org/obo/ENVO_00000004"/>
        <obo:RO_0001025 rdf:resource="http://purl.obolibrary.org/obo/GAZ_00010650"/>
        <obo:IAO_0000115>A district located in the southern part of Helmand Province, Afghanistan.</obo:IAO_0000115>
        <oboInOwl:hasOBONamespace>GAZ</oboInOwl:hasOBONamespace>
        <oboInOwl:id>GAZ:00021592</oboInOwl:id>
        <rdfs:label>Garmser District</rdfs:label>
    </owl:NamedIndividual>
    


    <!-- http://purl.obolibrary.org/obo/GAZ_00021593 -->

    <owl:NamedIndividual rdf:about="http://purl.obolibrary.org/obo/GAZ_00021593">
        <rdf:type rdf:resource="http://purl.obolibrary.org/obo/ENVO_00000004"/>
        <obo:RO_0001025 rdf:resource="http://purl.obolibrary.org/obo/GAZ_00010650"/>
        <obo:IAO_0000115>A district of Helmand Province, Afghanistan.</obo:IAO_0000115>
        <oboInOwl:hasOBONamespace>GAZ</oboInOwl:hasOBONamespace>
        <oboInOwl:id>GAZ:00021593</oboInOwl:id>
        <rdfs:label>Reg District</rdfs:label>
    </owl:NamedIndividual>
    


    <!-- http://purl.obolibrary.org/obo/GAZ_00021594 -->

    <owl:NamedIndividual rdf:about="http://purl.obolibrary.org/obo/GAZ_00021594">
        <rdf:type rdf:resource="http://purl.obolibrary.org/obo/ENVO_00000004"/>
        <obo:RO_0001025 rdf:resource="http://purl.obolibrary.org/obo/GAZ_00010650"/>
        <obo:IAO_0000115>A district located south to the Lashkargah District in Helmand Province, Afghanistan.</obo:IAO_0000115>
        <oboInOwl:hasOBONamespace>GAZ</oboInOwl:hasOBONamespace>
        <oboInOwl:id>GAZ:00021594</oboInOwl:id>
        <rdfs:label>Nawa-I-Barakzayi District</rdfs:label>
    </owl:NamedIndividual>
    


    <!-- http://purl.obolibrary.org/obo/GAZ_00021595 -->

    <owl:NamedIndividual rdf:about="http://purl.obolibrary.org/obo/GAZ_00021595">
        <rdf:type rdf:resource="http://purl.obolibrary.org/obo/ENVO_00000004"/>
        <obo:RO_0001025 rdf:resource="http://purl.obolibrary.org/obo/GAZ_00010650"/>
        <obo:IAO_0000115>A district in the west of Helmand Province, Afghanistan.</obo:IAO_0000115>
        <oboInOwl:hasOBONamespace>GAZ</oboInOwl:hasOBONamespace>
        <oboInOwl:id>GAZ:00021595</oboInOwl:id>
        <rdfs:label>Nad Ali District</rdfs:label>
    </owl:NamedIndividual>
    


    <!-- http://purl.obolibrary.org/obo/GAZ_00021596 -->

    <owl:NamedIndividual rdf:about="http://purl.obolibrary.org/obo/GAZ_00021596">
        <rdf:type rdf:resource="http://purl.obolibrary.org/obo/ENVO_00000004"/>
        <obo:RO_0001025 rdf:resource="http://purl.obolibrary.org/obo/GAZ_00010650"/>
        <obo:IAO_0000115>A district in the east of Helmand Province, Afghanistan.</obo:IAO_0000115>
        <oboInOwl:hasOBONamespace>GAZ</oboInOwl:hasOBONamespace>
        <oboInOwl:id>GAZ:00021596</oboInOwl:id>
        <rdfs:label>Sangin District</rdfs:label>
    </owl:NamedIndividual>
    


    <!-- http://purl.obolibrary.org/obo/GAZ_00021597 -->

    <owl:NamedIndividual rdf:about="http://purl.obolibrary.org/obo/GAZ_00021597">
        <rdf:type rdf:resource="http://purl.obolibrary.org/obo/ENVO_00000004"/>
        <obo:RO_0001025 rdf:resource="http://purl.obolibrary.org/obo/GAZ_00010650"/>
        <obo:IAO_0000115>A district in the north of Helmand Province, Afghanistan.</obo:IAO_0000115>
        <oboInOwl:hasOBONamespace>GAZ</oboInOwl:hasOBONamespace>
        <oboInOwl:id>GAZ:00021597</oboInOwl:id>
        <rdfs:label>Naw Zad District</rdfs:label>
    </owl:NamedIndividual>
    


    <!-- http://purl.obolibrary.org/obo/GAZ_00021598 -->

    <owl:NamedIndividual rdf:about="http://purl.obolibrary.org/obo/GAZ_00021598">
        <rdf:type rdf:resource="http://purl.obolibrary.org/obo/ENVO_00000004"/>
        <obo:RO_0001025 rdf:resource="http://purl.obolibrary.org/obo/GAZ_00010653"/>
        <obo:IAO_0000115>A district of Herat province in northwestern Afghanistan. It borders the nation of Iran to the west, Gulran District to the north, and Ghurian District to the south and east.</obo:IAO_0000115>
        <oboInOwl:hasOBONamespace>GAZ</oboInOwl:hasOBONamespace>
        <oboInOwl:id>GAZ:00021598</oboInOwl:id>
        <rdfs:label>Kohsan District</rdfs:label>
    </owl:NamedIndividual>
    


    <!-- http://purl.obolibrary.org/obo/GAZ_00021599 -->

    <owl:NamedIndividual rdf:about="http://purl.obolibrary.org/obo/GAZ_00021599">
        <obo:RO_0001025 rdf:resource="http://purl.obolibrary.org/obo/GAZ_00010653"/>
        <obo:IAO_0000115>A district the west of Herat Province, Afghanistan. It borders on Obe District to the north, Adraskan District to the west, Shindand District to the south and Ghor Province to the south and east.</obo:IAO_0000115>
        <oboInOwl:hasOBONamespace>GAZ</oboInOwl:hasOBONamespace>
        <oboInOwl:id>GAZ:00021599</oboInOwl:id>
        <rdfs:label>Farsi District</rdfs:label>
    </owl:NamedIndividual>
    


    <!-- http://purl.obolibrary.org/obo/GAZ_00021600 -->

    <owl:NamedIndividual rdf:about="http://purl.obolibrary.org/obo/GAZ_00021600">
        <rdf:type rdf:resource="http://purl.obolibrary.org/obo/ENVO_00000004"/>
        <obo:RO_0001025 rdf:resource="http://purl.obolibrary.org/obo/GAZ_00010653"/>
        <obo:IAO_0000115>A district of Herat province in northwestern Afghanistan. It surrounds Herat City and borders Kushk District to the north, Karukh District to the east, Guzara District to the south, and Zinda Jan District to the west.</obo:IAO_0000115>
        <oboInOwl:hasOBONamespace>GAZ</oboInOwl:hasOBONamespace>
        <oboInOwl:id>GAZ:00021600</oboInOwl:id>
        <rdfs:label>Injil District</rdfs:label>
    </owl:NamedIndividual>
    


    <!-- http://purl.obolibrary.org/obo/GAZ_00021601 -->

    <owl:NamedIndividual rdf:about="http://purl.obolibrary.org/obo/GAZ_00021601">
        <obo:RO_0001025 rdf:resource="http://purl.obolibrary.org/obo/GAZ_00010653"/>
        <obo:IAO_0000115>A district situated in the center of the Herat Province in Afghanistan, 10 km South to Herat. It borders with Injil District to the North, Pashtun Zarghun District to the East, Adraskan District to the South and Zinda Jan District to the West.</obo:IAO_0000115>
        <oboInOwl:hasOBONamespace>GAZ</oboInOwl:hasOBONamespace>
        <oboInOwl:id>GAZ:00021601</oboInOwl:id>
        <rdfs:label>Guzara District</rdfs:label>
    </owl:NamedIndividual>
    


    <!-- http://purl.obolibrary.org/obo/GAZ_00021602 -->

    <owl:NamedIndividual rdf:about="http://purl.obolibrary.org/obo/GAZ_00021602">
        <obo:RO_0001025 rdf:resource="http://purl.obolibrary.org/obo/GAZ_00010653"/>
        <obo:IAO_0000115>A district situated in Nort-Western part of Herat province, Afghanistan and borders Iran to the West, Turkmenistan to the North, Kushk District to the East, and Zinda Jan District and Kohsan District to the South.</obo:IAO_0000115>
        <oboInOwl:hasOBONamespace>GAZ</oboInOwl:hasOBONamespace>
        <oboInOwl:id>GAZ:00021602</oboInOwl:id>
        <rdfs:label>Gulran District</rdfs:label>
    </owl:NamedIndividual>
    


    <!-- http://purl.obolibrary.org/obo/GAZ_00021603 -->

    <owl:NamedIndividual rdf:about="http://purl.obolibrary.org/obo/GAZ_00021603">
        <rdf:type rdf:resource="http://purl.obolibrary.org/obo/ENVO_00000004"/>
        <obo:RO_0001025 rdf:resource="http://purl.obolibrary.org/obo/GAZ_00010653"/>
        <obo:IAO_0000115>A district located in the central part of the Herat Province in Afghanistan. It borders Gulran and Kushk districts to the North, Injil and Guzara districts to the East, Adraskan District to the South and Ghoryan and Kohsan districts to the West.</obo:IAO_0000115>
        <oboInOwl:hasOBONamespace>GAZ</oboInOwl:hasOBONamespace>
        <oboInOwl:id>GAZ:00021603</oboInOwl:id>
        <rdfs:label>Zinda Jan District</rdfs:label>
    </owl:NamedIndividual>
    


    <!-- http://purl.obolibrary.org/obo/GAZ_00021604 -->

    <owl:NamedIndividual rdf:about="http://purl.obolibrary.org/obo/GAZ_00021604">
        <rdf:type rdf:resource="http://purl.obolibrary.org/obo/ENVO_00000004"/>
        <obo:RO_0001025 rdf:resource="http://purl.obolibrary.org/obo/GAZ_00010653"/>
        <obo:IAO_0000115>A district of Herat province in northwestern Afghanistan. It is situated in the northern part of the province. It borders Kushk District to the west, the nation of Turkmenistan to the north, Badghis Province to the east, and Karukh District to the south.</obo:IAO_0000115>
        <oboInOwl:hasOBONamespace>GAZ</oboInOwl:hasOBONamespace>
        <oboInOwl:id>GAZ:00021604</oboInOwl:id>
        <rdfs:label>Kushki Kohna District</rdfs:label>
    </owl:NamedIndividual>
    


    <!-- http://purl.obolibrary.org/obo/GAZ_00021605 -->

    <owl:NamedIndividual rdf:about="http://purl.obolibrary.org/obo/GAZ_00021605">
        <obo:RO_0001025 rdf:resource="http://purl.obolibrary.org/obo/GAZ_00010653"/>
        <obo:IAO_0000115>A district situated in the central part of the Herat Province, Afghanistan in the valley of the Hari River. It borders with Karukh District to the North, Obe District to the east, Adraskan District to the south and Guzara District to the west.</obo:IAO_0000115>
        <oboInOwl:hasOBONamespace>GAZ</oboInOwl:hasOBONamespace>
        <oboInOwl:id>GAZ:00021605</oboInOwl:id>
        <rdfs:label>Pashtun Zarghun District</rdfs:label>
    </owl:NamedIndividual>
    


    <!-- http://purl.obolibrary.org/obo/GAZ_00021606 -->

    <owl:NamedIndividual rdf:about="http://purl.obolibrary.org/obo/GAZ_00021606">
        <obo:RO_0001025 rdf:resource="http://purl.obolibrary.org/obo/GAZ_00010653"/>
        <obo:IAO_0000115>A district situated in the southern part of the Herat Province in Afghanistan. It borders with Adraskan District to the North, Ghor Province to the East and Farah Province to the South and West.</obo:IAO_0000115>
        <oboInOwl:hasOBONamespace>GAZ</oboInOwl:hasOBONamespace>
        <oboInOwl:id>GAZ:00021606</oboInOwl:id>
        <rdfs:label>Shindand District</rdfs:label>
    </owl:NamedIndividual>
    


    <!-- http://purl.obolibrary.org/obo/GAZ_00021607 -->

    <owl:NamedIndividual rdf:about="http://purl.obolibrary.org/obo/GAZ_00021607">
        <obo:RO_0001025 rdf:resource="http://purl.obolibrary.org/obo/GAZ_00010653"/>
        <obo:IAO_0000115>A district situated in the northern part of Herat Province in Afghanistan. It borders Turkmenistan to the North, Gulran District to the West, Zinda Jan District, Injil District and Karukh District to the South and Kushki Kuhna District to the East.</obo:IAO_0000115>
        <oboInOwl:hasOBONamespace>GAZ</oboInOwl:hasOBONamespace>
        <oboInOwl:id>GAZ:00021607</oboInOwl:id>
        <rdfs:label>Kushk District</rdfs:label>
    </owl:NamedIndividual>
    


    <!-- http://purl.obolibrary.org/obo/GAZ_00021608 -->

    <owl:NamedIndividual rdf:about="http://purl.obolibrary.org/obo/GAZ_00021608">
        <rdf:type rdf:resource="http://purl.obolibrary.org/obo/ENVO_00000004"/>
        <obo:RO_0001025 rdf:resource="http://purl.obolibrary.org/obo/GAZ_00010653"/>
        <obo:IAO_0000115>A district in the northeast of Herat Province, Afghanistan. It borders on the north with Badghis Province, on the east with Chishti sharif District, on the southeast with Farsi District, on the south with Adraskan District, and on the west with Pashtun Zarghun and Karukh districts.</obo:IAO_0000115>
        <oboInOwl:hasOBONamespace>GAZ</oboInOwl:hasOBONamespace>
        <oboInOwl:id>GAZ:00021608</oboInOwl:id>
        <rdfs:label>Obe District</rdfs:label>
    </owl:NamedIndividual>
    


    <!-- http://purl.obolibrary.org/obo/GAZ_00021609 -->

    <owl:NamedIndividual rdf:about="http://purl.obolibrary.org/obo/GAZ_00021609">
        <rdf:type rdf:resource="http://purl.obolibrary.org/obo/ENVO_00000004"/>
        <obo:RO_0001025 rdf:resource="http://purl.obolibrary.org/obo/GAZ_00010653"/>
        <obo:IAO_0000115>A district in the central part of Herat Province in Afghanistan. It is bordered to the west by Iran, to the north by Ghoryan District, Zinda Jan District, Guzara District, Pashtun Zarghun District and Obe District, to the east by Farsi District and to the south by Shindand District.</obo:IAO_0000115>
        <oboInOwl:hasOBONamespace>GAZ</oboInOwl:hasOBONamespace>
        <oboInOwl:id>GAZ:00021609</oboInOwl:id>
        <rdfs:label>Adraskan District</rdfs:label>
    </owl:NamedIndividual>
    


    <!-- http://purl.obolibrary.org/obo/GAZ_00021610 -->

    <owl:NamedIndividual rdf:about="http://purl.obolibrary.org/obo/GAZ_00021610">
        <obo:RO_0001025 rdf:resource="http://purl.obolibrary.org/obo/GAZ_00010653"/>
        <obo:IAO_0000115>The most easterly district in Herat Province, Afghanistan, situated along the Hari River and one of its northern tributaries. It borders with Obe District to the west, Badghis Province to the north and Ghor Province to the east and south.</obo:IAO_0000115>
        <oboInOwl:hasOBONamespace>GAZ</oboInOwl:hasOBONamespace>
        <oboInOwl:id>GAZ:00021610</oboInOwl:id>
        <rdfs:label>Chishti Sharif District</rdfs:label>
    </owl:NamedIndividual>
    


    <!-- http://purl.obolibrary.org/obo/GAZ_00021611 -->

    <owl:NamedIndividual rdf:about="http://purl.obolibrary.org/obo/GAZ_00021611">
        <obo:RO_0001025 rdf:resource="http://purl.obolibrary.org/obo/GAZ_00010641"/>
        <obo:IAO_0000115>A desert district, situated in the Karakum Desert. It borders Faryab Province to the West, Khamyab District to the North, Mangajik District to the East and Sheberghan District to the South.</obo:IAO_0000115>
        <oboInOwl:hasOBONamespace>GAZ</oboInOwl:hasOBONamespace>
        <oboInOwl:id>GAZ:00021611</oboInOwl:id>
        <rdfs:label>Khwaja Du Koh District</rdfs:label>
    </owl:NamedIndividual>
    


    <!-- http://purl.obolibrary.org/obo/GAZ_00021612 -->

    <owl:NamedIndividual rdf:about="http://purl.obolibrary.org/obo/GAZ_00021612">
        <obo:RO_0001025 rdf:resource="http://purl.obolibrary.org/obo/GAZ_00010641"/>
        <obo:IAO_0000115>A district situated in the Eastern part of Jowzjan Province, Afghanistan. It borders Aqcha District to the West, Mardyan District to the North, Balkh Province to the East and Sar-e Pol Province to the South.</obo:IAO_0000115>
        <oboInOwl:hasOBONamespace>GAZ</oboInOwl:hasOBONamespace>
        <oboInOwl:id>GAZ:00021612</oboInOwl:id>
        <rdfs:label>Fayzabad District</rdfs:label>
    </owl:NamedIndividual>
    


    <!-- http://purl.obolibrary.org/obo/GAZ_00021613 -->

    <owl:NamedIndividual rdf:about="http://purl.obolibrary.org/obo/GAZ_00021613">
        <obo:RO_0001025 rdf:resource="http://purl.obolibrary.org/obo/GAZ_00010641"/>
        <obo:IAO_0000115>A district situated in the southern part of Jowzjan Province. It borders Faryab Province to the West, Khwaja du koh District to the North, Aqcha District to the East and Sar-e Pol Province.</obo:IAO_0000115>
        <oboInOwl:hasOBONamespace>GAZ</oboInOwl:hasOBONamespace>
        <oboInOwl:id>GAZ:00021613</oboInOwl:id>
        <rdfs:label>Shibirghan District</rdfs:label>
    </owl:NamedIndividual>
    


    <!-- http://purl.obolibrary.org/obo/GAZ_00021614 -->

    <owl:NamedIndividual rdf:about="http://purl.obolibrary.org/obo/GAZ_00021614">
        <obo:RO_0001025 rdf:resource="http://purl.obolibrary.org/obo/GAZ_00010635"/>
        <obo:IAO_0000115>A district situated in the southern part of Kabul Province in Afghanistan. Mussai district borders with Char Asiab District to the west, Bagrami District to the north, Khaki Jabbar District to the east and Lowgar Province to the south.</obo:IAO_0000115>
        <oboInOwl:hasOBONamespace>GAZ</oboInOwl:hasOBONamespace>
        <oboInOwl:id>GAZ:00021614</oboInOwl:id>
        <rdfs:label>Musayi District</rdfs:label>
    </owl:NamedIndividual>
    


    <!-- http://purl.obolibrary.org/obo/GAZ_00021615 -->

    <owl:NamedIndividual rdf:about="http://purl.obolibrary.org/obo/GAZ_00021615">
        <obo:RO_0001025 rdf:resource="http://purl.obolibrary.org/obo/GAZ_00010641"/>
        <obo:IAO_0000115>A district situated in the central part of Jowzjan Province in northern Afghanistan. It borders with Mardyan and Mingajik districts to the north, Sheberghan District to the West, Sar-e Pol Province to the south and Fayzabad District to the east.</obo:IAO_0000115>
        <oboInOwl:hasOBONamespace>GAZ</oboInOwl:hasOBONamespace>
        <oboInOwl:id>GAZ:00021615</oboInOwl:id>
        <rdfs:label>Aqcha District</rdfs:label>
    </owl:NamedIndividual>
    


    <!-- http://purl.obolibrary.org/obo/GAZ_00021616 -->

    <owl:NamedIndividual rdf:about="http://purl.obolibrary.org/obo/GAZ_00021616">
        <obo:RO_0001025 rdf:resource="http://purl.obolibrary.org/obo/GAZ_00010641"/>
        <obo:IAO_0000115>A frontier district in the province of Jowzjan in Afghanistan. It shares borders with Turkmenistan to the north and west, Khwaja du koh District to the south and the Mingajik and Qarqin districts to the east.</obo:IAO_0000115>
        <oboInOwl:hasOBONamespace>GAZ</oboInOwl:hasOBONamespace>
        <oboInOwl:id>GAZ:00021616</oboInOwl:id>
        <rdfs:label>Khamyab District</rdfs:label>
    </owl:NamedIndividual>
    


    <!-- http://purl.obolibrary.org/obo/GAZ_00021617 -->

    <owl:NamedIndividual rdf:about="http://purl.obolibrary.org/obo/GAZ_00021617">
        <rdf:type rdf:resource="http://purl.obolibrary.org/obo/ENVO_00000004"/>
        <obo:RO_0001025 rdf:resource="http://purl.obolibrary.org/obo/GAZ_00010635"/>
        <obo:IAO_0000115>A district of Kabul province in Afghanistan.</obo:IAO_0000115>
        <oboInOwl:hasOBONamespace>GAZ</oboInOwl:hasOBONamespace>
        <oboInOwl:id>GAZ:00021617</oboInOwl:id>
        <rdfs:label>Kabul District</rdfs:label>
    </owl:NamedIndividual>
    


    <!-- http://purl.obolibrary.org/obo/GAZ_00021618 -->

    <owl:NamedIndividual rdf:about="http://purl.obolibrary.org/obo/GAZ_00021618">
        <obo:RO_0001025 rdf:resource="http://purl.obolibrary.org/obo/GAZ_00010641"/>
        <obo:IAO_0000115>A district situated in the central part of Jowzjan Province, Afghanistan. It borders Khwaja du koh and Khamyab districts to the west, Qarqin District to the north, Mardyan District to the east and Aqcha District to the south.</obo:IAO_0000115>
        <oboInOwl:hasOBONamespace>GAZ</oboInOwl:hasOBONamespace>
        <oboInOwl:id>GAZ:00021618</oboInOwl:id>
        <rdfs:label>Mingajik District</rdfs:label>
    </owl:NamedIndividual>
    


    <!-- http://purl.obolibrary.org/obo/GAZ_00021619 -->

    <owl:NamedIndividual rdf:about="http://purl.obolibrary.org/obo/GAZ_00021619">
        <rdf:type rdf:resource="http://purl.obolibrary.org/obo/ENVO_00000004"/>
        <obo:RO_0001025 rdf:resource="http://purl.obolibrary.org/obo/GAZ_00010635"/>
        <obo:IAO_0000115>A district situated northeast of Kabul City in Afghanistan. Dih Sabz borders with Shakardara and Mir Bacha Kot districts to the west, Kalakan and Qarabagh districts to the north-west, Parvan Province to the north and east, Surobi to the southeast and Bagrami and Kabul districts to the south.</obo:IAO_0000115>
        <oboInOwl:hasOBONamespace>GAZ</oboInOwl:hasOBONamespace>
        <oboInOwl:id>GAZ:00021619</oboInOwl:id>
        <rdfs:label>Dih Sabz District</rdfs:label>
    </owl:NamedIndividual>
    


    <!-- http://purl.obolibrary.org/obo/GAZ_00021620 -->

    <owl:NamedIndividual rdf:about="http://purl.obolibrary.org/obo/GAZ_00021620">
        <obo:RO_0001025 rdf:resource="http://purl.obolibrary.org/obo/GAZ_00010641"/>
        <obo:IAO_0000115>A small boundary district in the northern part of Jowzjan Province, Afghanistan. It borders Turkmenistan to the North along the Amu Darya River, Khamyab District to the West, Mingajik and Mardyan districts to the South, and Balkh Province to the East.</obo:IAO_0000115>
        <oboInOwl:hasOBONamespace>GAZ</oboInOwl:hasOBONamespace>
        <oboInOwl:id>GAZ:00021620</oboInOwl:id>
        <rdfs:label>Qarqin District</rdfs:label>
    </owl:NamedIndividual>
    


    <!-- http://purl.obolibrary.org/obo/GAZ_00021621 -->

    <owl:NamedIndividual rdf:about="http://purl.obolibrary.org/obo/GAZ_00021621">
        <rdf:type rdf:resource="http://purl.obolibrary.org/obo/ENVO_00000004"/>
        <obo:RO_0001025 rdf:resource="http://purl.obolibrary.org/obo/GAZ_00010635"/>
        <obo:IAO_0000115>A district located in the northern part of Kabul Province, Afghanistan. It borders with Guldara District to the West, Qarabagh District to the North, Dih Sabz District to the East and Mir Bacha Kot District to the South.</obo:IAO_0000115>
        <oboInOwl:hasOBONamespace>GAZ</oboInOwl:hasOBONamespace>
        <oboInOwl:id>GAZ:00021621</oboInOwl:id>
        <rdfs:label>Kalakan District</rdfs:label>
    </owl:NamedIndividual>
    


    <!-- http://purl.obolibrary.org/obo/GAZ_00021622 -->

    <owl:NamedIndividual rdf:about="http://purl.obolibrary.org/obo/GAZ_00021622">
        <obo:RO_0001025 rdf:resource="http://purl.obolibrary.org/obo/GAZ_00010641"/>
        <obo:IAO_0000115>The most Southwestern district in the Jowzjan Province, Afghanistan. It borders with Sheberghan District to North-East, Sar-e Pol Province to the West and Faryab Province to the South and West.</obo:IAO_0000115>
        <oboInOwl:hasOBONamespace>GAZ</oboInOwl:hasOBONamespace>
        <oboInOwl:id>GAZ:00021622</oboInOwl:id>
        <rdfs:label>Darzab District</rdfs:label>
    </owl:NamedIndividual>
    


    <!-- http://purl.obolibrary.org/obo/GAZ_00021623 -->

    <owl:NamedIndividual rdf:about="http://purl.obolibrary.org/obo/GAZ_00021623">
        <obo:RO_0001025 rdf:resource="http://purl.obolibrary.org/obo/GAZ_00010641"/>
        <obo:IAO_0000115>A district situated in the central Eastern part of the Jowzjan Province, Afghanistan. It borders Mingajik District to the West, Qarqin District to North, Balkh Province and Fayzabad District to the East and Aqcha District to the South.</obo:IAO_0000115>
        <oboInOwl:hasOBONamespace>GAZ</oboInOwl:hasOBONamespace>
        <oboInOwl:id>GAZ:00021623</oboInOwl:id>
        <rdfs:label>Mardyan District</rdfs:label>
    </owl:NamedIndividual>
    


    <!-- http://purl.obolibrary.org/obo/GAZ_00021624 -->

    <owl:NamedIndividual rdf:about="http://purl.obolibrary.org/obo/GAZ_00021624">
        <rdf:type rdf:resource="http://purl.obolibrary.org/obo/ENVO_00000004"/>
        <obo:RO_0001025 rdf:resource="http://purl.obolibrary.org/obo/GAZ_00010642"/>
        <obo:IAO_0000115>A district in Kandahar Province, Afghanistan. It is located about 35 km west of Kandahar city. The district borders with Helmand Province to the South-West, Maywand District to the West, Khakrez District to the North, Arghandab, Kandahar and Daman districts to the East and Reg District to the South.</obo:IAO_0000115>
        <oboInOwl:hasOBONamespace>GAZ</oboInOwl:hasOBONamespace>
        <oboInOwl:id>GAZ:00021624</oboInOwl:id>
        <rdfs:label>Panjwaii District</rdfs:label>
    </owl:NamedIndividual>
    


    <!-- http://purl.obolibrary.org/obo/GAZ_00021625 -->

    <owl:NamedIndividual rdf:about="http://purl.obolibrary.org/obo/GAZ_00021625">
        <obo:RO_0001025 rdf:resource="http://purl.obolibrary.org/obo/GAZ_00010635"/>
        <obo:IAO_0000115>A mountainous district situated in the eastern part of Kabul Province in Afghanistan. Khaki Jabbar district borders with Lowgar Province and Musayi District to the west, Bagrami and Surobi districts to the north, and Nangarhar Province to the east.</obo:IAO_0000115>
        <oboInOwl:hasOBONamespace>GAZ</oboInOwl:hasOBONamespace>
        <oboInOwl:id>GAZ:00021625</oboInOwl:id>
        <rdfs:label>Khaki Jabbar District</rdfs:label>
    </owl:NamedIndividual>
    


    <!-- http://purl.obolibrary.org/obo/GAZ_00021626 -->

    <owl:NamedIndividual rdf:about="http://purl.obolibrary.org/obo/GAZ_00021626">
        <obo:RO_0001025 rdf:resource="http://purl.obolibrary.org/obo/GAZ_00010635"/>
        <obo:IAO_0000115>A district situated in the southern part of the Kabul province in Afghanistan. Char Asiab district borders with Lowgar province to the south, Wardak province to the west, Paghman District to the north-west, Kabul to the north, and Bagrami and Mussahi districts to the west.</obo:IAO_0000115>
        <oboInOwl:hasOBONamespace>GAZ</oboInOwl:hasOBONamespace>
        <oboInOwl:id>GAZ:00021626</oboInOwl:id>
        <rdfs:label>Chahar Asyab District</rdfs:label>
    </owl:NamedIndividual>
    


    <!-- http://purl.obolibrary.org/obo/GAZ_00021627 -->

    <owl:NamedIndividual rdf:about="http://purl.obolibrary.org/obo/GAZ_00021627">
        <obo:RO_0001025 rdf:resource="http://purl.obolibrary.org/obo/GAZ_00010635"/>
        <obo:IAO_0000115>A district situated in the western part of Kabul Province in Afghanistan. Paghman district borders with Wardak and Parwan provinces to the west, Shakardara District to the north, Kabul to the east and Char Asiab District to the south-east.</obo:IAO_0000115>
        <oboInOwl:hasOBONamespace>GAZ</oboInOwl:hasOBONamespace>
        <oboInOwl:id>GAZ:00021627</oboInOwl:id>
        <rdfs:label>Paghman District</rdfs:label>
    </owl:NamedIndividual>
    


    <!-- http://purl.obolibrary.org/obo/GAZ_00021628 -->

    <owl:NamedIndividual rdf:about="http://purl.obolibrary.org/obo/GAZ_00021628">
        <rdf:type rdf:resource="http://purl.obolibrary.org/obo/ENVO_00000004"/>
        <obo:RO_0001025 rdf:resource="http://purl.obolibrary.org/obo/GAZ_00010635"/>
        <obo:IAO_0000115>A district located in the northwestern part of Kabul Province in Afghanistan. Guldara district borders with Parvan Province to the west, Istalif District to the north, Qarabagh, Kalakan and Mir Bacha Kot districts to the east, and Shakardara District to the south.</obo:IAO_0000115>
        <oboInOwl:hasOBONamespace>GAZ</oboInOwl:hasOBONamespace>
        <oboInOwl:id>GAZ:00021628</oboInOwl:id>
        <rdfs:label>Guldara District</rdfs:label>
    </owl:NamedIndividual>
    


    <!-- http://purl.obolibrary.org/obo/GAZ_00021629 -->

    <owl:NamedIndividual rdf:about="http://purl.obolibrary.org/obo/GAZ_00021629">
        <rdf:type rdf:resource="http://purl.obolibrary.org/obo/ENVO_00000004"/>
        <obo:RO_0001025 rdf:resource="http://purl.obolibrary.org/obo/GAZ_00010635"/>
        <obo:IAO_0000115>A district located in the northwestern part of the Kabul Province in Afghanistan. Istalif district borders with Parvan Province to the north and west, Qarabagh District to the east and Guldara District to the south. The district headquarter is the village of Istalif, situated in the southeastern part of the district.</obo:IAO_0000115>
        <oboInOwl:hasOBONamespace>GAZ</oboInOwl:hasOBONamespace>
        <oboInOwl:id>GAZ:00021629</oboInOwl:id>
        <rdfs:label>Istalif District</rdfs:label>
    </owl:NamedIndividual>
    


    <!-- http://purl.obolibrary.org/obo/GAZ_00021630 -->

    <owl:NamedIndividual rdf:about="http://purl.obolibrary.org/obo/GAZ_00021630">
        <obo:RO_0001025 rdf:resource="http://purl.obolibrary.org/obo/GAZ_00010635"/>
        <obo:IAO_0000115>A district situated in the north-eastern part of the Kabul Province of Afghanistan, approximately 70 km north of Kabul City. Surobi district borders with Bagrami and Deh Sabz districts to the west, Parvan and Kapisa provinces to the north, Laghman Province to the east, and Nangarhar Province and Khaki Jabbar District to the south.</obo:IAO_0000115>
        <oboInOwl:hasOBONamespace>GAZ</oboInOwl:hasOBONamespace>
        <oboInOwl:id>GAZ:00021630</oboInOwl:id>
        <rdfs:label>Surobi District</rdfs:label>
    </owl:NamedIndividual>
    


    <!-- http://purl.obolibrary.org/obo/GAZ_00021631 -->

    <owl:NamedIndividual rdf:about="http://purl.obolibrary.org/obo/GAZ_00021631">
        <obo:RO_0001025 rdf:resource="http://purl.obolibrary.org/obo/GAZ_00010635"/>
        <obo:IAO_0000115>A district situated in the central part of the Kabul Province in Afghanistan. Shakar Dara district borders with Parvan Province to the west, Guldara District to the north, Mir Bacha Kot, Deh Sabz and Kabul districts to the east, and Paghman District to the south.</obo:IAO_0000115>
        <oboInOwl:hasOBONamespace>GAZ</oboInOwl:hasOBONamespace>
        <oboInOwl:id>GAZ:00021631</oboInOwl:id>
        <rdfs:label>Shakar Dara District</rdfs:label>
    </owl:NamedIndividual>
    


    <!-- http://purl.obolibrary.org/obo/GAZ_00021632 -->

    <owl:NamedIndividual rdf:about="http://purl.obolibrary.org/obo/GAZ_00021632">
        <obo:RO_0001025 rdf:resource="http://purl.obolibrary.org/obo/GAZ_00010642"/>
        <obo:IAO_0000115>A district situated in the nortwestern part of Kandahar Province, Afghanistan. It borders Helmand Province to the West, Oruzgan Province and Naish District to the North, Khakrez District to the East and Maywand District to the South.</obo:IAO_0000115>
        <oboInOwl:hasOBONamespace>GAZ</oboInOwl:hasOBONamespace>
        <oboInOwl:id>GAZ:00021632</oboInOwl:id>
        <rdfs:label>Ghorak District</rdfs:label>
    </owl:NamedIndividual>
    


    <!-- http://purl.obolibrary.org/obo/GAZ_00021633 -->

    <owl:NamedIndividual rdf:about="http://purl.obolibrary.org/obo/GAZ_00021633">
        <rdf:type rdf:resource="http://purl.obolibrary.org/obo/ENVO_00000004"/>
        <obo:RO_0001025 rdf:resource="http://purl.obolibrary.org/obo/GAZ_00010635"/>
        <obo:IAO_0000115>A district located in the central part of Kabul Province in Afghanistan. The district borders with Kabul to the west, De Sabz to the north, Surobi to the east, and Khaki Jabbar, Musayi and Char Asiab districts to the South.</obo:IAO_0000115>
        <oboInOwl:hasOBONamespace>GAZ</oboInOwl:hasOBONamespace>
        <oboInOwl:id>GAZ:00021633</oboInOwl:id>
        <rdfs:label>Bagrami District</rdfs:label>
    </owl:NamedIndividual>
    


    <!-- http://purl.obolibrary.org/obo/GAZ_00021634 -->

    <owl:NamedIndividual rdf:about="http://purl.obolibrary.org/obo/GAZ_00021634">
        <obo:RO_0001025 rdf:resource="http://purl.obolibrary.org/obo/GAZ_00010635"/>
        <obo:IAO_0000115>A district situated in the central part of Kabul Province in Afghanistan. Mir Bacha Kot district borders Shakardara District to the west, Guldara and Kalakan districts to the north, and Deh Sabz District to the east.</obo:IAO_0000115>
        <oboInOwl:hasOBONamespace>GAZ</oboInOwl:hasOBONamespace>
        <oboInOwl:id>GAZ:00021634</oboInOwl:id>
        <rdfs:label>Mir Bacha Kot District</rdfs:label>
    </owl:NamedIndividual>
    


    <!-- http://purl.obolibrary.org/obo/GAZ_00021635 -->

    <owl:NamedIndividual rdf:about="http://purl.obolibrary.org/obo/GAZ_00021635">
        <rdf:type rdf:resource="http://purl.obolibrary.org/obo/ENVO_00000004"/>
        <obo:RO_0001025 rdf:resource="http://purl.obolibrary.org/obo/GAZ_00010635"/>
        <obo:IAO_0000115>A district located 50 km north of Kabul City in Afghanistan, and 20 km southeast of Bagram Air base. Qarabagh district borders with Guldara and Istalif districts to the north, Parvan Province to the south and east, and Deh Sabz and Kalakan districts to the south.</obo:IAO_0000115>
        <oboInOwl:hasOBONamespace>GAZ</oboInOwl:hasOBONamespace>
        <oboInOwl:id>GAZ:00021635</oboInOwl:id>
        <rdfs:label>Qarabagh District</rdfs:label>
    </owl:NamedIndividual>
    


    <!-- http://purl.obolibrary.org/obo/GAZ_00021636 -->

    <owl:NamedIndividual rdf:about="http://purl.obolibrary.org/obo/GAZ_00021636">
        <rdf:type rdf:resource="http://purl.obolibrary.org/obo/ENVO_00000004"/>
        <obo:RO_0001025 rdf:resource="http://purl.obolibrary.org/obo/GAZ_00010642"/>
        <obo:IAO_0000115>A district in the central part of Kandahar Province, Afghanistan. It borders with Panjwai and Khakrez districts to the West, Shah Wali Kot District to the North and East and Kandahar District to the East and South.</obo:IAO_0000115>
        <oboInOwl:hasOBONamespace>GAZ</oboInOwl:hasOBONamespace>
        <oboInOwl:id>GAZ:00021636</oboInOwl:id>
        <rdfs:label>Arghandab District</rdfs:label>
    </owl:NamedIndividual>
    


    <!-- http://purl.obolibrary.org/obo/GAZ_00021637 -->

    <owl:NamedIndividual rdf:about="http://purl.obolibrary.org/obo/GAZ_00021637">
        <obo:RO_0001025 rdf:resource="http://purl.obolibrary.org/obo/GAZ_00010642"/>
        <obo:IAO_0000115>A district situated in the central part of the Kandahar Province, Afghanistan, surrounding the city of Kandahar. It borders with Panjwai District to the West, Arghandab District to the North, Shah Wali Kot District to the North-East and Daman District to the East and South.</obo:IAO_0000115>
        <oboInOwl:hasOBONamespace>GAZ</oboInOwl:hasOBONamespace>
        <oboInOwl:id>GAZ:00021637</oboInOwl:id>
        <rdfs:label>Kandahar District</rdfs:label>
    </owl:NamedIndividual>
    


    <!-- http://purl.obolibrary.org/obo/GAZ_00021638 -->

    <owl:NamedIndividual rdf:about="http://purl.obolibrary.org/obo/GAZ_00021638">
        <obo:RO_0001025 rdf:resource="http://purl.obolibrary.org/obo/GAZ_00010637"/>
        <obo:IAO_0000115>A district situated in the northwestern part of Kapisa Province, Afghanistan. It borders Kohistan Districts to the West, Parvan Province to the North, Nejrab District to the East and Mahmud Raqi District to the South.</obo:IAO_0000115>
        <oboInOwl:hasOBONamespace>GAZ</oboInOwl:hasOBONamespace>
        <oboInOwl:id>GAZ:00021638</oboInOwl:id>
        <rdfs:label>Koh Band District</rdfs:label>
    </owl:NamedIndividual>
    


    <!-- http://purl.obolibrary.org/obo/GAZ_00021639 -->

    <owl:NamedIndividual rdf:about="http://purl.obolibrary.org/obo/GAZ_00021639">
        <obo:RO_0001025 rdf:resource="http://purl.obolibrary.org/obo/GAZ_00010642"/>
        <obo:IAO_0000115>A district situated in the central part of the Kandahar Province, Afghanistan. It borders Panjwai and Kandahar districts to the West, Shah Wali Kot District to the North, Zabul Province to the North-East, Arghistan and Spin Boldak districts to the East and Reg District to the South.</obo:IAO_0000115>
        <oboInOwl:hasOBONamespace>GAZ</oboInOwl:hasOBONamespace>
        <oboInOwl:id>GAZ:00021639</oboInOwl:id>
        <rdfs:label>Daman District</rdfs:label>
    </owl:NamedIndividual>
    


    <!-- http://purl.obolibrary.org/obo/GAZ_00021640 -->

    <owl:NamedIndividual rdf:about="http://purl.obolibrary.org/obo/GAZ_00021640">
        <rdf:type rdf:resource="http://purl.obolibrary.org/obo/ENVO_00000004"/>
        <obo:RO_0001025 rdf:resource="http://purl.obolibrary.org/obo/GAZ_00010642"/>
        <obo:IAO_0000115>A district in Kandahar Province, Afghanistan. The district was created from territories taken from Maywand and Panjwai districts.</obo:IAO_0000115>
        <oboInOwl:hasOBONamespace>GAZ</oboInOwl:hasOBONamespace>
        <oboInOwl:id>GAZ:00021640</oboInOwl:id>
        <rdfs:label>Zhari District</rdfs:label>
    </owl:NamedIndividual>
    


    <!-- http://purl.obolibrary.org/obo/GAZ_00021641 -->

    <owl:NamedIndividual rdf:about="http://purl.obolibrary.org/obo/GAZ_00021641">
        <obo:RO_0001025 rdf:resource="http://purl.obolibrary.org/obo/GAZ_00010642"/>
        <obo:IAO_0000115>A district situated in the southern part of Kandahar Province, Afghanistan. It borders Helmand Province to the West, Panjwai and Daman districts to the North, Shorabak District to the East and Pakistan to the South.</obo:IAO_0000115>
        <oboInOwl:hasOBONamespace>GAZ</oboInOwl:hasOBONamespace>
        <oboInOwl:id>GAZ:00021641</oboInOwl:id>
        <rdfs:label>Reg District</rdfs:label>
    </owl:NamedIndividual>
    


    <!-- http://purl.obolibrary.org/obo/GAZ_00021642 -->

    <owl:NamedIndividual rdf:about="http://purl.obolibrary.org/obo/GAZ_00021642">
        <obo:RO_0001025 rdf:resource="http://purl.obolibrary.org/obo/GAZ_00010642"/>
        <obo:IAO_0000115>A district situated in the northeastern part of Kandahar Province, Afghanistan. It borders Spin Boldak District to the South and West, Daman District to the West, Zabul Province to the North, Maruf District to the East and Pakistan to the East and South.</obo:IAO_0000115>
        <oboInOwl:hasOBONamespace>GAZ</oboInOwl:hasOBONamespace>
        <oboInOwl:id>GAZ:00021642</oboInOwl:id>
        <rdfs:label>Arghistan District</rdfs:label>
    </owl:NamedIndividual>
    


    <!-- http://purl.obolibrary.org/obo/GAZ_00021643 -->

    <owl:NamedIndividual rdf:about="http://purl.obolibrary.org/obo/GAZ_00021643">
        <obo:RO_0001025 rdf:resource="http://purl.obolibrary.org/obo/GAZ_00010642"/>
        <obo:IAO_0000115>A district situated in the northern part of Kandahar Province, Afghanistan. It borders Ghorak District to the West,Maywand and Panjwai districts to the South, Arghandab and Shah Wali Kot districts to the East and Naish District to the North.</obo:IAO_0000115>
        <oboInOwl:hasOBONamespace>GAZ</oboInOwl:hasOBONamespace>
        <oboInOwl:id>GAZ:00021643</oboInOwl:id>
        <rdfs:label>Khakrez District</rdfs:label>
    </owl:NamedIndividual>
    


    <!-- http://purl.obolibrary.org/obo/GAZ_00021644 -->

    <owl:NamedIndividual rdf:about="http://purl.obolibrary.org/obo/GAZ_00021644">
        <obo:RO_0001025 rdf:resource="http://purl.obolibrary.org/obo/GAZ_00010637"/>
        <obo:IAO_0000115>A district situated in the central part of Kapisa Province, Afghanistan. It is located in a green valley supported by the springs from Hindu Kush mountains and about 120 km north of Kabul. It borders Mahmud Raqi and Koh Band districts to the west, Parvan Province to the north, Laghman Province and Alasay District to the east and Tagab District to the south.</obo:IAO_0000115>
        <oboInOwl:hasOBONamespace>GAZ</oboInOwl:hasOBONamespace>
        <oboInOwl:id>GAZ:00021644</oboInOwl:id>
        <rdfs:label>Nijrab District</rdfs:label>
    </owl:NamedIndividual>
    


    <!-- http://purl.obolibrary.org/obo/GAZ_00021645 -->

    <owl:NamedIndividual rdf:about="http://purl.obolibrary.org/obo/GAZ_00021645">
        <obo:RO_0001025 rdf:resource="http://purl.obolibrary.org/obo/GAZ_00010637"/>
        <obo:IAO_0000115>A district situated in the western part of Kapisa Province, Afghanistan. It borders with Parvan Province to the South and with other districts from the Kapisa Province: Nejrab District and the former Kohistan District to the North and Tagab District to the South-East.</obo:IAO_0000115>
        <oboInOwl:hasOBONamespace>GAZ</oboInOwl:hasOBONamespace>
        <oboInOwl:id>GAZ:00021645</oboInOwl:id>
        <rdfs:label>Mahmud Raqi District</rdfs:label>
    </owl:NamedIndividual>
    


    <!-- http://purl.obolibrary.org/obo/GAZ_00021646 -->

    <owl:NamedIndividual rdf:about="http://purl.obolibrary.org/obo/GAZ_00021646">
        <rdf:type rdf:resource="http://purl.obolibrary.org/obo/ENVO_00000004"/>
        <obo:RO_0001025 rdf:resource="http://purl.obolibrary.org/obo/GAZ_00010642"/>
        <obo:IAO_0000115>A district, situated in the southeastern part of Kandahar Province, Afghanistan, 110 km South and East of Kandahar. It borders Reg District to the West, Spin Boldak District to the North and Pakistan to the East and South.</obo:IAO_0000115>
        <oboInOwl:hasOBONamespace>GAZ</oboInOwl:hasOBONamespace>
        <oboInOwl:id>GAZ:00021646</oboInOwl:id>
        <rdfs:label>Shorabak District</rdfs:label>
    </owl:NamedIndividual>
    


    <!-- http://purl.obolibrary.org/obo/GAZ_00021647 -->

    <owl:NamedIndividual rdf:about="http://purl.obolibrary.org/obo/GAZ_00021647">
        <rdf:type rdf:resource="http://purl.obolibrary.org/obo/ENVO_00000004"/>
        <obo:RO_0001025 rdf:resource="http://purl.obolibrary.org/obo/GAZ_00010642"/>
        <obo:IAO_0000115>A district in the eastern part of Kandahar Province, Afghanistan. It borders Daman District to the West, Arghistan District to the North, Qilla Abdullah District Pakistan to the East and Shorabak District to the South.</obo:IAO_0000115>
        <oboInOwl:hasOBONamespace>GAZ</oboInOwl:hasOBONamespace>
        <oboInOwl:id>GAZ:00021647</oboInOwl:id>
        <rdfs:label>Spin Boldak District</rdfs:label>
    </owl:NamedIndividual>
    


    <!-- http://purl.obolibrary.org/obo/GAZ_00021648 -->

    <owl:NamedIndividual rdf:about="http://purl.obolibrary.org/obo/GAZ_00021648">
        <rdf:type rdf:resource="http://purl.obolibrary.org/obo/ENVO_00000004"/>
        <obo:RO_0001025 rdf:resource="http://purl.obolibrary.org/obo/GAZ_00010642"/>
        <obo:IAO_0000115>A district in Kandahar Province, Afghanistan. It borders Arghistan District to the West, Zabul Province to the North and Pakistan to the East and South.</obo:IAO_0000115>
        <oboInOwl:hasOBONamespace>GAZ</oboInOwl:hasOBONamespace>
        <oboInOwl:id>GAZ:00021648</oboInOwl:id>
        <rdfs:label>Maruf District</rdfs:label>
    </owl:NamedIndividual>
    


    <!-- http://purl.obolibrary.org/obo/GAZ_00021649 -->

    <owl:NamedIndividual rdf:about="http://purl.obolibrary.org/obo/GAZ_00021649">
        <obo:RO_0001025 rdf:resource="http://purl.obolibrary.org/obo/GAZ_00010642"/>
        <obo:IAO_0000115>A district situated in the northern part of Kandahar Province, Afghanistan. It borders Khakrez District to the West, Naish District and Oruzgan Province to the North, Zabul Province to the East and Daman and Arghandab districts to the South.</obo:IAO_0000115>
        <oboInOwl:hasOBONamespace>GAZ</oboInOwl:hasOBONamespace>
        <oboInOwl:id>GAZ:00021649</oboInOwl:id>
        <rdfs:label>Shah Wali Kot District</rdfs:label>
    </owl:NamedIndividual>
    


    <!-- http://purl.obolibrary.org/obo/GAZ_00021650 -->

    <owl:NamedIndividual rdf:about="http://purl.obolibrary.org/obo/GAZ_00021650">
        <obo:RO_0001025 rdf:resource="http://purl.obolibrary.org/obo/GAZ_00010642"/>
        <obo:IAO_0000115>A district situated in the western part of the Kandahar Province, Afghanistan. It borders Helmand Province to the West, Ghorak District to the North, Khakrez District to the North-East and Panjwai District to the East and South.</obo:IAO_0000115>
        <oboInOwl:hasOBONamespace>GAZ</oboInOwl:hasOBONamespace>
        <oboInOwl:id>GAZ:00021650</oboInOwl:id>
        <rdfs:label>Maywand District</rdfs:label>
    </owl:NamedIndividual>
    


    <!-- http://purl.obolibrary.org/obo/GAZ_00021652 -->

    <owl:NamedIndividual rdf:about="http://purl.obolibrary.org/obo/GAZ_00021652">
        <obo:RO_0001025 rdf:resource="http://purl.obolibrary.org/obo/GAZ_00010637"/>
        <obo:IAO_0000115>A district situated in the eastern part of Kapisa Province, Afghanistan. It borders Tagab District to the South and East, Nejrab District to the North and Laghman Province to the East.</obo:IAO_0000115>
        <oboInOwl:hasOBONamespace>GAZ</oboInOwl:hasOBONamespace>
        <oboInOwl:id>GAZ:00021652</oboInOwl:id>
        <rdfs:label>Alasay District</rdfs:label>
    </owl:NamedIndividual>
    


    <!-- http://purl.obolibrary.org/obo/GAZ_00021653 -->

    <owl:NamedIndividual rdf:about="http://purl.obolibrary.org/obo/GAZ_00021653">
        <obo:RO_0001025 rdf:resource="http://purl.obolibrary.org/obo/GAZ_00010637"/>
        <obo:IAO_0000115>A district situated in the eastern part of Kapisa Province, Afghanistan. It borders with Parvan Province to the West, Mahmud Raqi and Nijrab to the North, Alasay District to the East and Kabul Province to the South-East.</obo:IAO_0000115>
        <oboInOwl:hasOBONamespace>GAZ</oboInOwl:hasOBONamespace>
        <oboInOwl:id>GAZ:00021653</oboInOwl:id>
        <rdfs:label>Tagab District</rdfs:label>
    </owl:NamedIndividual>
    


    <!-- http://purl.obolibrary.org/obo/GAZ_00021654 -->

    <owl:NamedIndividual rdf:about="http://purl.obolibrary.org/obo/GAZ_00021654">
        <obo:RO_0001025 rdf:resource="http://purl.obolibrary.org/obo/GAZ_00010634"/>
        <obo:IAO_0000115>A district situated in the central and eastern part of Khost Province, Afghanistan. It borders with Mandozi and Nadir Shah Kot districts to the West, Musa Khel District to the North-West, Sabari District to the North, Tere Zayi District to the North and East, Pakistan to the South and Gurbuz District to the South ad West.</obo:IAO_0000115>
        <oboInOwl:hasOBONamespace>GAZ</oboInOwl:hasOBONamespace>
        <oboInOwl:id>GAZ:00021654</oboInOwl:id>
        <rdfs:label>Khost (Matun) District</rdfs:label>
    </owl:NamedIndividual>
    


    <!-- http://purl.obolibrary.org/obo/GAZ_00021655 -->

    <owl:NamedIndividual rdf:about="http://purl.obolibrary.org/obo/GAZ_00021655">
        <obo:RO_0001025 rdf:resource="http://purl.obolibrary.org/obo/GAZ_00010634"/>
        <obo:IAO_0000115>A district situated in the southern part of Khost Province, Afghanistan. It borders with Tani District to the West, Mando Zayi and Khost districts to the North and Pakistan to the East and South.</obo:IAO_0000115>
        <oboInOwl:hasOBONamespace>GAZ</oboInOwl:hasOBONamespace>
        <oboInOwl:id>GAZ:00021655</oboInOwl:id>
        <rdfs:label>Gurbuz District</rdfs:label>
    </owl:NamedIndividual>
    


    <!-- http://purl.obolibrary.org/obo/GAZ_00021656 -->

    <owl:NamedIndividual rdf:about="http://purl.obolibrary.org/obo/GAZ_00021656">
        <obo:RO_0001025 rdf:resource="http://purl.obolibrary.org/obo/GAZ_00010634"/>
        <obo:IAO_0000115>One of the districts of Khost Province, Afghanistan. It is situated in the North East of the province. It borders with Khost and Sabari districts to the West, Bak District to the North and Pakistan to the East.</obo:IAO_0000115>
        <oboInOwl:hasOBONamespace>GAZ</oboInOwl:hasOBONamespace>
        <oboInOwl:id>GAZ:00021656</oboInOwl:id>
        <rdfs:label>Tere Zayi District</rdfs:label>
    </owl:NamedIndividual>
    


    <!-- http://purl.obolibrary.org/obo/GAZ_00021657 -->

    <owl:NamedIndividual rdf:about="http://purl.obolibrary.org/obo/GAZ_00021657">
        <obo:RO_0001025 rdf:resource="http://purl.obolibrary.org/obo/GAZ_00010634"/>
        <obo:IAO_0000115>A district situated in the northern part of the Khost Province, Afghanistan. It borders with Paktia Province to the North, Sabari District to the East, Khost (Matun) District to the South, Nadir Shah Kot District to the South-West and Qalandar District to the West.</obo:IAO_0000115>
        <oboInOwl:hasOBONamespace>GAZ</oboInOwl:hasOBONamespace>
        <oboInOwl:id>GAZ:00021657</oboInOwl:id>
        <rdfs:label>Musa Khel District</rdfs:label>
    </owl:NamedIndividual>
    


    <!-- http://purl.obolibrary.org/obo/GAZ_00021658 -->

    <owl:NamedIndividual rdf:about="http://purl.obolibrary.org/obo/GAZ_00021658">
        <rdf:type rdf:resource="http://purl.obolibrary.org/obo/ENVO_00000004"/>
        <obo:RO_0001025 rdf:resource="http://purl.obolibrary.org/obo/GAZ_00010634"/>
        <obo:IAO_0000115>A district located in the northeastern part of Khost Province, Afghanistan. It borders with Bak District to the West, Paktia Province to the North and Pakistan to the North and East.</obo:IAO_0000115>
        <oboInOwl:hasOBONamespace>GAZ</oboInOwl:hasOBONamespace>
        <oboInOwl:id>GAZ:00021658</oboInOwl:id>
        <rdfs:label>Jaji Maydan District</rdfs:label>
    </owl:NamedIndividual>
    


    <!-- http://purl.obolibrary.org/obo/GAZ_00021659 -->

    <owl:NamedIndividual rdf:about="http://purl.obolibrary.org/obo/GAZ_00021659">
        <obo:RO_0001025 rdf:resource="http://purl.obolibrary.org/obo/GAZ_00010634"/>
        <obo:IAO_0000115>A district situated in the western part of Khost Province, Afghanistan. It borders with Paktia Province to the West, Musa Khel District to the North and East and Nadir Shah Kot District to the South.</obo:IAO_0000115>
        <oboInOwl:hasOBONamespace>GAZ</oboInOwl:hasOBONamespace>
        <oboInOwl:id>GAZ:00021659</oboInOwl:id>
        <rdfs:label>Qalandar District</rdfs:label>
    </owl:NamedIndividual>
    


    <!-- http://purl.obolibrary.org/obo/GAZ_00021660 -->

    <owl:NamedIndividual rdf:about="http://purl.obolibrary.org/obo/GAZ_00021660">
        <obo:RO_0001025 rdf:resource="http://purl.obolibrary.org/obo/GAZ_00010634"/>
        <obo:IAO_0000115>A district situated in the central part of Khost Province, Afghanistan. It borders with Nadir Shah Kot District to the North and West, Khost (Matun) District to the East, Gurbuz District to the South-West and Tani District to the South.</obo:IAO_0000115>
        <oboInOwl:hasOBONamespace>GAZ</oboInOwl:hasOBONamespace>
        <oboInOwl:id>GAZ:00021660</oboInOwl:id>
        <rdfs:label>Mando Zayi District</rdfs:label>
    </owl:NamedIndividual>
    


    <!-- http://purl.obolibrary.org/obo/GAZ_00021661 -->

    <owl:NamedIndividual rdf:about="http://purl.obolibrary.org/obo/GAZ_00021661">
        <obo:RO_0001025 rdf:resource="http://purl.obolibrary.org/obo/GAZ_00010634"/>
        <obo:IAO_0000115>A district situated in the southern part of Khost Province, Afghanistan. It borders with Spera District to the West, Nadir Shah Kot and Mando Zayi to the North, Gurbuz District to the East and Pakistan to the South.</obo:IAO_0000115>
        <oboInOwl:hasOBONamespace>GAZ</oboInOwl:hasOBONamespace>
        <oboInOwl:id>GAZ:00021661</oboInOwl:id>
        <rdfs:label>Tani District</rdfs:label>
    </owl:NamedIndividual>
    


    <!-- http://purl.obolibrary.org/obo/GAZ_00021662 -->

    <owl:NamedIndividual rdf:about="http://purl.obolibrary.org/obo/GAZ_00021662">
        <obo:RO_0001025 rdf:resource="http://purl.obolibrary.org/obo/GAZ_00010634"/>
        <obo:IAO_0000115>A district situated in the northern part of Khost Province, Afghanistan. It borders with Sabari District to the west, Paktia Province and Jaji Maydan District to the North, Pakistan to the East and Tere Zayi District to the South.</obo:IAO_0000115>
        <oboInOwl:hasOBONamespace>GAZ</oboInOwl:hasOBONamespace>
        <oboInOwl:id>GAZ:00021662</oboInOwl:id>
        <rdfs:label>Bak District</rdfs:label>
    </owl:NamedIndividual>
    


    <!-- http://purl.obolibrary.org/obo/GAZ_00021663 -->

    <owl:NamedIndividual rdf:about="http://purl.obolibrary.org/obo/GAZ_00021663">
        <obo:RO_0001025 rdf:resource="http://purl.obolibrary.org/obo/GAZ_00010634"/>
        <obo:IAO_0000115>A district situated in the western part of Khost Province, Afghanistan. It borders with Paktia Province and Shamal District to the West, Qalandar District to the North, Musa Khel District to the North-East, Khost (Matun) District to the East, Mando Zayi District to the South-east and Tani and Spera districts to the South.</obo:IAO_0000115>
        <oboInOwl:hasOBONamespace>GAZ</oboInOwl:hasOBONamespace>
        <oboInOwl:id>GAZ:00021663</oboInOwl:id>
        <rdfs:label>Nadir Shah Kot District</rdfs:label>
    </owl:NamedIndividual>
    


    <!-- http://purl.obolibrary.org/obo/GAZ_00021664 -->

    <owl:NamedIndividual rdf:about="http://purl.obolibrary.org/obo/GAZ_00021664">
        <obo:RO_0001025 rdf:resource="http://purl.obolibrary.org/obo/GAZ_00010634"/>
        <obo:IAO_0000115>A district situated in the northern part of Khost Province, Afghanistan. It borders on: Musa Khel District to the West, Paktia Province to the North, Bak District to the East and Tere Zayi and Khost districts to the South.</obo:IAO_0000115>
        <oboInOwl:hasOBONamespace>GAZ</oboInOwl:hasOBONamespace>
        <oboInOwl:id>GAZ:00021664</oboInOwl:id>
        <rdfs:label>Sabari District</rdfs:label>
    </owl:NamedIndividual>
    


    <!-- http://purl.obolibrary.org/obo/GAZ_00021665 -->

    <owl:NamedIndividual rdf:about="http://purl.obolibrary.org/obo/GAZ_00021665">
        <obo:RO_0001025 rdf:resource="http://purl.obolibrary.org/obo/GAZ_00010634"/>
        <obo:IAO_0000115>A district situated in the most southwestern part of Khost Province, Afghanistan. It borders with Paktia Province to the South and West, Shamal District to the North. To the East it borders with Nadir Shah Kot and Tani districts and Pakistan.</obo:IAO_0000115>
        <oboInOwl:hasOBONamespace>GAZ</oboInOwl:hasOBONamespace>
        <oboInOwl:id>GAZ:00021665</oboInOwl:id>
        <rdfs:label>Spera District</rdfs:label>
    </owl:NamedIndividual>
    


    <!-- http://purl.obolibrary.org/obo/GAZ_00021666 -->

    <owl:NamedIndividual rdf:about="http://purl.obolibrary.org/obo/GAZ_00021666">
        <obo:RO_0001025 rdf:resource="http://purl.obolibrary.org/obo/GAZ_00010632"/>
        <obo:IAO_0000115>A district situated in the central part of Kunar Province, Afghanistan.</obo:IAO_0000115>
        <oboInOwl:hasOBONamespace>GAZ</oboInOwl:hasOBONamespace>
        <oboInOwl:id>GAZ:00021666</oboInOwl:id>
        <rdfs:label>Chawkay District</rdfs:label>
    </owl:NamedIndividual>
    


    <!-- http://purl.obolibrary.org/obo/GAZ_00021667 -->

    <owl:NamedIndividual rdf:about="http://purl.obolibrary.org/obo/GAZ_00021667">
        <obo:RO_0001025 rdf:resource="http://purl.obolibrary.org/obo/GAZ_00010632"/>
        <obo:IAO_0000115>A district situated in the northeastern part of Kunar Province, Afghanistan. It borders with Asadabad district to the south-west, Nuristan Province to the north-west, Nari district to the north-east and Dangam district to the south-east.</obo:IAO_0000115>
        <oboInOwl:hasOBONamespace>GAZ</oboInOwl:hasOBONamespace>
        <oboInOwl:id>GAZ:00021667</oboInOwl:id>
        <rdfs:label>Bar Kunar District</rdfs:label>
    </owl:NamedIndividual>
    


    <!-- http://purl.obolibrary.org/obo/GAZ_00021668 -->

    <owl:NamedIndividual rdf:about="http://purl.obolibrary.org/obo/GAZ_00021668">
        <obo:RO_0001025 rdf:resource="http://purl.obolibrary.org/obo/GAZ_00010632"/>
        <obo:IAO_0000115>A district situated in the central part of Kunar Province, Afghanistan. It borders Pakistan to the South.</obo:IAO_0000115>
        <oboInOwl:hasOBONamespace>GAZ</oboInOwl:hasOBONamespace>
        <oboInOwl:id>GAZ:00021668</oboInOwl:id>
        <rdfs:label>Sirkanay District</rdfs:label>
    </owl:NamedIndividual>
    


    <!-- http://purl.obolibrary.org/obo/GAZ_00021669 -->

    <owl:NamedIndividual rdf:about="http://purl.obolibrary.org/obo/GAZ_00021669">
        <obo:RO_0001025 rdf:resource="http://purl.obolibrary.org/obo/GAZ_00010632"/>
        <obo:IAO_0000115>One of 15 districts in Kunar Province, Afghanistan. It includes the city of Asadabad - the district center, close the Kunar River. It is situated in the central part of the province and borders with Dara-I-Pech district and Nuristan Province to the West, Bar Kunar, Dangam, Marawara and Sirkanay districts to the East and Narang wa Badil district to the South.</obo:IAO_0000115>
        <oboInOwl:hasOBONamespace>GAZ</oboInOwl:hasOBONamespace>
        <oboInOwl:id>GAZ:00021669</oboInOwl:id>
        <rdfs:label>Asadabad District</rdfs:label>
    </owl:NamedIndividual>
    


    <!-- http://purl.obolibrary.org/obo/GAZ_00021670 -->

    <owl:NamedIndividual rdf:about="http://purl.obolibrary.org/obo/GAZ_00021670">
        <obo:RO_0001025 rdf:resource="http://purl.obolibrary.org/obo/GAZ_00010632"/>
        <obo:IAO_0000115>A district situated in the western part of Kunar Province, Afghanistan and borders Nuristan Province. The district was split and Shaygal Wa Shiltan district was created from it.</obo:IAO_0000115>
        <oboInOwl:hasOBONamespace>GAZ</oboInOwl:hasOBONamespace>
        <oboInOwl:id>GAZ:00021670</oboInOwl:id>
        <rdfs:label>Chapa Dara District</rdfs:label>
    </owl:NamedIndividual>
    


    <!-- http://purl.obolibrary.org/obo/GAZ_00021671 -->

    <owl:NamedIndividual rdf:about="http://purl.obolibrary.org/obo/GAZ_00021671">
        <obo:RO_0001025 rdf:resource="http://purl.obolibrary.org/obo/GAZ_00010632"/>
        <obo:IAO_0000115>A district situated in the central part of Kunar Province, Afghanistan south of Asadabad. It is surrounded by high mountains and the Kunar River.</obo:IAO_0000115>
        <oboInOwl:hasOBONamespace>GAZ</oboInOwl:hasOBONamespace>
        <oboInOwl:id>GAZ:00021671</oboInOwl:id>
        <rdfs:label>Narang District</rdfs:label>
    </owl:NamedIndividual>
    


    <!-- http://purl.obolibrary.org/obo/GAZ_00021672 -->

    <owl:NamedIndividual rdf:about="http://purl.obolibrary.org/obo/GAZ_00021672">
        <obo:RO_0001025 rdf:resource="http://purl.obolibrary.org/obo/GAZ_00010632"/>
        <obo:IAO_0000115>A boundary mountainous district in the most eastern part of Kunar Province in Afghanistan. It borders Bar Kunar district to the West, Nuristan Province to the North, Pakistan to the East and Dangam district to the South.</obo:IAO_0000115>
        <oboInOwl:hasOBONamespace>GAZ</oboInOwl:hasOBONamespace>
        <oboInOwl:id>GAZ:00021672</oboInOwl:id>
        <rdfs:label>Nari District</rdfs:label>
    </owl:NamedIndividual>
    


    <!-- http://purl.obolibrary.org/obo/GAZ_00021673 -->

    <owl:NamedIndividual rdf:about="http://purl.obolibrary.org/obo/GAZ_00021673">
        <obo:RO_0001025 rdf:resource="http://purl.obolibrary.org/obo/GAZ_00010632"/>
        <obo:IAO_0000115>One of the 15 districts in Kunar Province, Afghanistan, bordering Pakistan to the East. It borders with Sirkanay district to the West, Asadabad district to the North-West and Dangam district to North-East.</obo:IAO_0000115>
        <oboInOwl:hasOBONamespace>GAZ</oboInOwl:hasOBONamespace>
        <oboInOwl:id>GAZ:00021673</oboInOwl:id>
        <rdfs:label>Marawara District</rdfs:label>
    </owl:NamedIndividual>
    


    <!-- http://purl.obolibrary.org/obo/GAZ_00021674 -->

    <owl:NamedIndividual rdf:about="http://purl.obolibrary.org/obo/GAZ_00021674">
        <obo:RO_0001025 rdf:resource="http://purl.obolibrary.org/obo/GAZ_00010632"/>
        <obo:IAO_0000115>A district situated in the eastern end of Kunar Province, Afghanistan. It borders Marawara district to the West, Asadabad district to the North-West, Bar Kunar district to the North, Nari district to the North-East and Pakistan to the East and South.</obo:IAO_0000115>
        <oboInOwl:hasOBONamespace>GAZ</oboInOwl:hasOBONamespace>
        <oboInOwl:id>GAZ:00021674</oboInOwl:id>
        <rdfs:label>Dangam District</rdfs:label>
    </owl:NamedIndividual>
    


    <!-- http://purl.obolibrary.org/obo/GAZ_00021676 -->

    <owl:NamedIndividual rdf:about="http://purl.obolibrary.org/obo/GAZ_00021676">
        <obo:RO_0001025 rdf:resource="http://purl.obolibrary.org/obo/GAZ_00010632"/>
        <obo:IAO_0000115>A district situated in the western part of Kunar Province, Afghanistan, 90 Km West from Asadabad, and is near Jalalabad city. It borders Nangarhar Province to the West and South, Chapa Dara district to the North and Chawkay and Khas Kunar districts to the East.</obo:IAO_0000115>
        <oboInOwl:hasOBONamespace>GAZ</oboInOwl:hasOBONamespace>
        <oboInOwl:id>GAZ:00021676</oboInOwl:id>
        <rdfs:label>Nurgal District</rdfs:label>
    </owl:NamedIndividual>
    


    <!-- http://purl.obolibrary.org/obo/GAZ_00021677 -->

    <owl:NamedIndividual rdf:about="http://purl.obolibrary.org/obo/GAZ_00021677">
        <obo:RO_0001025 rdf:resource="http://purl.obolibrary.org/obo/GAZ_00010632"/>
        <obo:IAO_0000115>The largest district in the Kunar Province, Afghanistan. It is situated in the southern part of the province and borders with Nangarhar Province to the South and Pakistan to the East.</obo:IAO_0000115>
        <oboInOwl:hasOBONamespace>GAZ</oboInOwl:hasOBONamespace>
        <oboInOwl:id>GAZ:00021677</oboInOwl:id>
        <rdfs:label>Khas Kunar District</rdfs:label>
    </owl:NamedIndividual>
    


    <!-- http://purl.obolibrary.org/obo/GAZ_00021678 -->

    <owl:NamedIndividual rdf:about="http://purl.obolibrary.org/obo/GAZ_00021678">
        <obo:RO_0001025 rdf:resource="http://purl.obolibrary.org/obo/GAZ_00010628"/>
        <obo:IAO_0000115>A district situated in the northwestern part of Kunduz Province in Afghanistan. It borders with Khan Abad and Kunduz districts to the South-West, Imam Sahib District to the North-West, Tajikistan to the Nort and Takhar Province to the East.</obo:IAO_0000115>
        <oboInOwl:hasOBONamespace>GAZ</oboInOwl:hasOBONamespace>
        <oboInOwl:id>GAZ:00021678</oboInOwl:id>
        <rdfs:label>Archi District</rdfs:label>
    </owl:NamedIndividual>
    


    <!-- http://purl.obolibrary.org/obo/GAZ_00021679 -->

    <owl:NamedIndividual rdf:about="http://purl.obolibrary.org/obo/GAZ_00021679">
        <obo:RO_0001025 rdf:resource="http://purl.obolibrary.org/obo/GAZ_00010628"/>
        <obo:IAO_0000115>A district situated in the southern part of Kunduz Province, Afghanistan. It borders with Baghlan Province to the South, Chahar dara District to the West, Kunduz and Khan Abad districts to the North and Takhar Province to the East.</obo:IAO_0000115>
        <oboInOwl:hasOBONamespace>GAZ</oboInOwl:hasOBONamespace>
        <oboInOwl:id>GAZ:00021679</oboInOwl:id>
        <rdfs:label>Aliabad District</rdfs:label>
    </owl:NamedIndividual>
    


    <!-- http://purl.obolibrary.org/obo/GAZ_00021680 -->

    <owl:NamedIndividual rdf:about="http://purl.obolibrary.org/obo/GAZ_00021680">
        <obo:RO_0001025 rdf:resource="http://purl.obolibrary.org/obo/GAZ_00010628"/>
        <obo:IAO_0000115>A district situated in the western part of Kunduz Province, Northern Afghanistan. It borders with Balkh Province to the West, Tajikistan to the North along the Panj, Vakhsh and Amu Darya rivers. To the East it borders with Imam Sahib District and to the South with Kunduz and Chahar dara districts.</obo:IAO_0000115>
        <oboInOwl:hasOBONamespace>GAZ</oboInOwl:hasOBONamespace>
        <oboInOwl:id>GAZ:00021680</oboInOwl:id>
        <rdfs:label>Qala-I-Zal District</rdfs:label>
    </owl:NamedIndividual>
    


    <!-- http://purl.obolibrary.org/obo/GAZ_00021681 -->

    <owl:NamedIndividual rdf:about="http://purl.obolibrary.org/obo/GAZ_00021681">
        <obo:RO_0001025 rdf:resource="http://purl.obolibrary.org/obo/GAZ_00010628"/>
        <obo:IAO_0000115>A district situated in the center of Kunduz Province in Northern Afghanistan, around the provincial capital-the city of Kunduz. It borders with Chahar dara District to the West, Qalay-I-Zal and Imam Sahib districts to the North, Archi and Khan Abad districts to the East and Ali abad District to the South.</obo:IAO_0000115>
        <oboInOwl:hasOBONamespace>GAZ</oboInOwl:hasOBONamespace>
        <oboInOwl:id>GAZ:00021681</oboInOwl:id>
        <rdfs:label>Kunduz District</rdfs:label>
    </owl:NamedIndividual>
    


    <!-- http://purl.obolibrary.org/obo/GAZ_00021682 -->

    <owl:NamedIndividual rdf:about="http://purl.obolibrary.org/obo/GAZ_00021682">
        <obo:RO_0001025 rdf:resource="http://purl.obolibrary.org/obo/GAZ_00010628"/>
        <obo:IAO_0000115>A district situated in the central part of Kunduz Province in Northern Afghanistan. It has borders with Qalay-I-Zal District to the west, Kunduz District to the north-east, Ali abad District to the west and Baghlan and Samangan provinces to the south.</obo:IAO_0000115>
        <oboInOwl:hasOBONamespace>GAZ</oboInOwl:hasOBONamespace>
        <oboInOwl:id>GAZ:00021682</oboInOwl:id>
        <rdfs:label>Chahar Dara District</rdfs:label>
    </owl:NamedIndividual>
    


    <!-- http://purl.obolibrary.org/obo/GAZ_00021683 -->

    <owl:NamedIndividual rdf:about="http://purl.obolibrary.org/obo/GAZ_00021683">
        <obo:RO_0001025 rdf:resource="http://purl.obolibrary.org/obo/GAZ_00010628"/>
        <obo:IAO_0000115>A district situated in the northern part of Kunduz Province, Afghanistan. It borders with Qalay-I-Zal District to the West, Tajikistan to the North (along the Panj river), with Archi District to the East and Kunduz District to the South.</obo:IAO_0000115>
        <oboInOwl:hasOBONamespace>GAZ</oboInOwl:hasOBONamespace>
        <oboInOwl:id>GAZ:00021683</oboInOwl:id>
        <rdfs:label>Imam Sahib District</rdfs:label>
    </owl:NamedIndividual>
    


    <!-- http://purl.obolibrary.org/obo/GAZ_00021684 -->

    <owl:NamedIndividual rdf:about="http://purl.obolibrary.org/obo/GAZ_00021684">
        <obo:RO_0001025 rdf:resource="http://purl.obolibrary.org/obo/GAZ_00010628"/>
        <obo:IAO_0000115>A district situated in the eastern part of Kunduz Province, Afghanistan. It borders with Kunduz District to the West, Archi District to the North-East, Takhar Province to the East and Ali abad District to the South.</obo:IAO_0000115>
        <oboInOwl:hasOBONamespace>GAZ</oboInOwl:hasOBONamespace>
        <oboInOwl:id>GAZ:00021684</oboInOwl:id>
        <rdfs:label>Khan Abad District</rdfs:label>
    </owl:NamedIndividual>
    


    <!-- http://purl.obolibrary.org/obo/GAZ_00021685 -->

    <owl:NamedIndividual rdf:about="http://purl.obolibrary.org/obo/GAZ_00021685">
        <rdf:type rdf:resource="http://purl.obolibrary.org/obo/ENVO_00000004"/>
        <obo:RO_0001025 rdf:resource="http://purl.obolibrary.org/obo/GAZ_00010630"/>
        <obo:IAO_0000115>A district in the east of Nangarhar Province, Afghanistan, bordering Pakistan.</obo:IAO_0000115>
        <oboInOwl:hasOBONamespace>GAZ</oboInOwl:hasOBONamespace>
        <oboInOwl:id>GAZ:00021685</oboInOwl:id>
        <rdfs:label>Muhmand Dara District</rdfs:label>
    </owl:NamedIndividual>
    


    <!-- http://purl.obolibrary.org/obo/GAZ_00021686 -->

    <owl:NamedIndividual rdf:about="http://purl.obolibrary.org/obo/GAZ_00021686">
        <rdf:type rdf:resource="http://purl.obolibrary.org/obo/ENVO_00000004"/>
        <obo:RO_0001025 rdf:resource="http://purl.obolibrary.org/obo/GAZ_00010633"/>
        <obo:IAO_0000115>A district in Lowgar Province.</obo:IAO_0000115>
        <oboInOwl:hasOBONamespace>GAZ</oboInOwl:hasOBONamespace>
        <oboInOwl:id>GAZ:00021686</oboInOwl:id>
        <rdfs:label>Puli Alam District</rdfs:label>
    </owl:NamedIndividual>
    


    <!-- http://purl.obolibrary.org/obo/GAZ_00021687 -->

    <owl:NamedIndividual rdf:about="http://purl.obolibrary.org/obo/GAZ_00021687">
        <obo:RO_0001025 rdf:resource="http://purl.obolibrary.org/obo/GAZ_00010627"/>
        <obo:IAO_0000115>The largest district in Laghman Province, and is located 30 Km from the provincial centre - Mihtarlam. It borders with Mihtarlam District to the North, Alingar District to the North-East, Nangarhar Province to the South and Kabul Province to the West.</obo:IAO_0000115>
        <oboInOwl:hasOBONamespace>GAZ</oboInOwl:hasOBONamespace>
        <oboInOwl:id>GAZ:00021687</oboInOwl:id>
        <rdfs:label>Qarghayi District</rdfs:label>
    </owl:NamedIndividual>
    


    <!-- http://purl.obolibrary.org/obo/GAZ_00021688 -->

    <owl:NamedIndividual rdf:about="http://purl.obolibrary.org/obo/GAZ_00021688">
        <obo:RO_0001025 rdf:resource="http://purl.obolibrary.org/obo/GAZ_00010633"/>
        <obo:IAO_0000115>A district situated in the southern part of Lowgar Province, Afghanistan. Kharwar District has been created from the former big Charkh District.</obo:IAO_0000115>
        <oboInOwl:hasOBONamespace>GAZ</oboInOwl:hasOBONamespace>
        <oboInOwl:id>GAZ:00021688</oboInOwl:id>
        <rdfs:label>Charkh District</rdfs:label>
    </owl:NamedIndividual>
    


    <!-- http://purl.obolibrary.org/obo/GAZ_00021689 -->

    <owl:NamedIndividual rdf:about="http://purl.obolibrary.org/obo/GAZ_00021689">
        <rdf:type rdf:resource="http://purl.obolibrary.org/obo/ENVO_00000004"/>
        <obo:RO_0001025 rdf:resource="http://purl.obolibrary.org/obo/GAZ_00010630"/>
        <obo:IAO_0000115>A district in the west of Nangarhar Province, Afghanistan. It has a short (approximately 5 km) stretch of border with Pakistan.</obo:IAO_0000115>
        <oboInOwl:hasOBONamespace>GAZ</oboInOwl:hasOBONamespace>
        <oboInOwl:id>GAZ:00021689</oboInOwl:id>
        <rdfs:label>Sherzad District</rdfs:label>
    </owl:NamedIndividual>
    


    <!-- http://purl.obolibrary.org/obo/GAZ_00021690 -->

    <owl:NamedIndividual rdf:about="http://purl.obolibrary.org/obo/GAZ_00021690">
        <rdf:type rdf:resource="http://purl.obolibrary.org/obo/ENVO_00000004"/>
        <obo:RO_0001025 rdf:resource="http://purl.obolibrary.org/obo/GAZ_00010630"/>
        <obo:IAO_0000115>A district in the east of Nangarhar Province, Afghanistan, bordering Pakistan.</obo:IAO_0000115>
        <oboInOwl:hasOBONamespace>GAZ</oboInOwl:hasOBONamespace>
        <oboInOwl:id>GAZ:00021690</oboInOwl:id>
        <rdfs:label>Lal Pur District</rdfs:label>
    </owl:NamedIndividual>
    


    <!-- http://purl.obolibrary.org/obo/GAZ_00021691 -->

    <owl:NamedIndividual rdf:about="http://purl.obolibrary.org/obo/GAZ_00021691">
        <rdf:type rdf:resource="http://purl.obolibrary.org/obo/ENVO_00000004"/>
        <obo:RO_0001025 rdf:resource="http://purl.obolibrary.org/obo/GAZ_00010630"/>
        <obo:IAO_0000115>A district in the north of Nangarhar Province, Afghanistan.</obo:IAO_0000115>
        <oboInOwl:hasOBONamespace>GAZ</oboInOwl:hasOBONamespace>
        <oboInOwl:id>GAZ:00021691</oboInOwl:id>
        <rdfs:label>Surkh Rod District</rdfs:label>
    </owl:NamedIndividual>
    


    <!-- http://purl.obolibrary.org/obo/GAZ_00021692 -->

    <owl:NamedIndividual rdf:about="http://purl.obolibrary.org/obo/GAZ_00021692">
        <rdf:type rdf:resource="http://purl.obolibrary.org/obo/ENVO_00000004"/>
        <obo:RO_0001025 rdf:resource="http://purl.obolibrary.org/obo/GAZ_00010630"/>
        <obo:IAO_0000115>A district in Nangarhar Province, Afghanistan.</obo:IAO_0000115>
        <oboInOwl:hasOBONamespace>GAZ</oboInOwl:hasOBONamespace>
        <oboInOwl:id>GAZ:00021692</oboInOwl:id>
        <rdfs:label>Shinwar District</rdfs:label>
    </owl:NamedIndividual>
    


    <!-- http://purl.obolibrary.org/obo/GAZ_00021693 -->

    <owl:NamedIndividual rdf:about="http://purl.obolibrary.org/obo/GAZ_00021693">
        <rdf:type rdf:resource="http://purl.obolibrary.org/obo/ENVO_00000004"/>
        <obo:RO_0001025 rdf:resource="http://purl.obolibrary.org/obo/GAZ_00010627"/>
        <obo:IAO_0000115>A district located approximately 74 km from Mehterlam, the provincial centre of Laghman Province. It is a mountainous district and borders Nuristan Province to the North and North-East, Alingar District to the East, Alishing District to the South and Kapisa and Parwan provinces to the West.</obo:IAO_0000115>
        <oboInOwl:hasOBONamespace>GAZ</oboInOwl:hasOBONamespace>
        <oboInOwl:id>GAZ:00021693</oboInOwl:id>
        <rdfs:label>Dawlat Shah District</rdfs:label>
    </owl:NamedIndividual>
    


    <!-- http://purl.obolibrary.org/obo/GAZ_00021694 -->

    <owl:NamedIndividual rdf:about="http://purl.obolibrary.org/obo/GAZ_00021694">
        <rdf:type rdf:resource="http://purl.obolibrary.org/obo/ENVO_00000004"/>
        <obo:RO_0001025 rdf:resource="http://purl.obolibrary.org/obo/GAZ_00010630"/>
        <obo:IAO_0000115>A district in the south-east of Nangarhar Province, Afghanistan.</obo:IAO_0000115>
        <oboInOwl:hasOBONamespace>GAZ</oboInOwl:hasOBONamespace>
        <oboInOwl:id>GAZ:00021694</oboInOwl:id>
        <rdfs:label>Nazyan District</rdfs:label>
    </owl:NamedIndividual>
    


    <!-- http://purl.obolibrary.org/obo/GAZ_00021695 -->

    <owl:NamedIndividual rdf:about="http://purl.obolibrary.org/obo/GAZ_00021695">
        <rdf:type rdf:resource="http://purl.obolibrary.org/obo/ENVO_00000004"/>
        <obo:RO_0001025 rdf:resource="http://purl.obolibrary.org/obo/GAZ_00010627"/>
        <obo:IAO_0000115>A district located in 21 km from Mihtarlam, the provincial centre of Laghman Province, and borders Kabul Province. It borders with Kabul and Kapisa provinces to the West, Dawlat Shah District to the North, Alingar District to the East and Mihtarlam District to the South.</obo:IAO_0000115>
        <oboInOwl:hasOBONamespace>GAZ</oboInOwl:hasOBONamespace>
        <oboInOwl:id>GAZ:00021695</oboInOwl:id>
        <rdfs:label>Alishing District</rdfs:label>
    </owl:NamedIndividual>
    


    <!-- http://purl.obolibrary.org/obo/GAZ_00021696 -->

    <owl:NamedIndividual rdf:about="http://purl.obolibrary.org/obo/GAZ_00021696">
        <rdf:type rdf:resource="http://purl.obolibrary.org/obo/ENVO_00000004"/>
        <obo:RO_0001025 rdf:resource="http://purl.obolibrary.org/obo/GAZ_00010627"/>
        <obo:IAO_0000115>A district located approximately 27 km from Mehtarlam, the provincial capital of Laghman Province and borders with Alishing and Dawlat Shah districts to the West, Nuristan Province to the North, Kunar and Nangarhar provinces to the East and Qarghayi and Mihtarlam districts to the South.</obo:IAO_0000115>
        <oboInOwl:hasOBONamespace>GAZ</oboInOwl:hasOBONamespace>
        <oboInOwl:id>GAZ:00021696</oboInOwl:id>
        <rdfs:label>Alingar District</rdfs:label>
    </owl:NamedIndividual>
    


    <!-- http://purl.obolibrary.org/obo/GAZ_00021697 -->

    <owl:NamedIndividual rdf:about="http://purl.obolibrary.org/obo/GAZ_00021697">
        <rdf:type rdf:resource="http://purl.obolibrary.org/obo/ENVO_00000004"/>
        <obo:RO_0001025 rdf:resource="http://purl.obolibrary.org/obo/GAZ_00010627"/>
        <obo:IAO_0000115>A district located in the center of Laghman Province and consists of the urban centre and provincial capital Mihtarlam and 24 major villages and 269 sub-villages. It borders with Kabul Province to the West, Alishing and Alingar districts to the North and Qarghayi District to the East and South.</obo:IAO_0000115>
        <oboInOwl:hasOBONamespace>GAZ</oboInOwl:hasOBONamespace>
        <oboInOwl:id>GAZ:00021697</oboInOwl:id>
        <rdfs:label>Mihtarlam District</rdfs:label>
    </owl:NamedIndividual>
    


    <!-- http://purl.obolibrary.org/obo/GAZ_00021698 -->

    <owl:NamedIndividual rdf:about="http://purl.obolibrary.org/obo/GAZ_00021698">
        <rdf:type rdf:resource="http://purl.obolibrary.org/obo/ENVO_00000004"/>
        <obo:RO_0001025 rdf:resource="http://purl.obolibrary.org/obo/GAZ_00010633"/>
        <obo:IAO_0000115>A district of Lowgar Province, Afghanistan.</obo:IAO_0000115>
        <oboInOwl:hasOBONamespace>GAZ</oboInOwl:hasOBONamespace>
        <oboInOwl:id>GAZ:00021698</oboInOwl:id>
        <rdfs:label>Khushi District</rdfs:label>
    </owl:NamedIndividual>
    


    <!-- http://purl.obolibrary.org/obo/GAZ_00021699 -->

    <owl:NamedIndividual rdf:about="http://purl.obolibrary.org/obo/GAZ_00021699">
        <obo:RO_0001025 rdf:resource="http://purl.obolibrary.org/obo/GAZ_00010633"/>
        <obo:IAO_0000115>A district situated in the western part of Lowgar Province, Afghanistan. It borders with Wardak Province to the West and North-West, Pul-i-Alam District to the North and East and Kharwar and Charkh districts to the South.</obo:IAO_0000115>
        <oboInOwl:hasOBONamespace>GAZ</oboInOwl:hasOBONamespace>
        <oboInOwl:id>GAZ:00021699</oboInOwl:id>
        <rdfs:label>Baraki Barak District</rdfs:label>
    </owl:NamedIndividual>
    


    <!-- http://purl.obolibrary.org/obo/GAZ_00021700 -->

    <owl:NamedIndividual rdf:about="http://purl.obolibrary.org/obo/GAZ_00021700">
        <rdf:type rdf:resource="http://purl.obolibrary.org/obo/ENVO_00000004"/>
        <obo:RO_0001025 rdf:resource="http://purl.obolibrary.org/obo/GAZ_00010630"/>
        <obo:IAO_0000115>A district in the centre of Nangarhar Province, Afghanistan, south of Jalalabad.</obo:IAO_0000115>
        <oboInOwl:hasOBONamespace>GAZ</oboInOwl:hasOBONamespace>
        <oboInOwl:id>GAZ:00021700</oboInOwl:id>
        <rdfs:label>Rodat District</rdfs:label>
    </owl:NamedIndividual>
    


    <!-- http://purl.obolibrary.org/obo/GAZ_00021701 -->

    <owl:NamedIndividual rdf:about="http://purl.obolibrary.org/obo/GAZ_00021701">
        <rdf:type rdf:resource="http://purl.obolibrary.org/obo/ENVO_00000004"/>
        <obo:RO_0001025 rdf:resource="http://purl.obolibrary.org/obo/GAZ_00010630"/>
        <obo:IAO_0000115>A district in the south-east of Nangarhar Province, Afghanistan, bordering Pakistan.</obo:IAO_0000115>
        <oboInOwl:hasOBONamespace>GAZ</oboInOwl:hasOBONamespace>
        <oboInOwl:id>GAZ:00021701</oboInOwl:id>
        <rdfs:label>Pachir Wa Agam District</rdfs:label>
    </owl:NamedIndividual>
    


    <!-- http://purl.obolibrary.org/obo/GAZ_00021702 -->

    <owl:NamedIndividual rdf:about="http://purl.obolibrary.org/obo/GAZ_00021702">
        <rdf:type rdf:resource="http://purl.obolibrary.org/obo/ENVO_00000004"/>
        <obo:RO_0001025 rdf:resource="http://purl.obolibrary.org/obo/GAZ_00010633"/>
        <obo:IAO_0000115>A district of Lowgar Province, Afghanistan.</obo:IAO_0000115>
        <oboInOwl:hasOBONamespace>GAZ</oboInOwl:hasOBONamespace>
        <oboInOwl:id>GAZ:00021702</oboInOwl:id>
        <rdfs:label>Muhammed Agha District</rdfs:label>
    </owl:NamedIndividual>
    


    <!-- http://purl.obolibrary.org/obo/GAZ_00021703 -->

    <owl:NamedIndividual rdf:about="http://purl.obolibrary.org/obo/GAZ_00021703">
        <rdf:type rdf:resource="http://purl.obolibrary.org/obo/ENVO_00000004"/>
        <obo:RO_0001025 rdf:resource="http://purl.obolibrary.org/obo/GAZ_00010631"/>
        <obo:IAO_0000115>A district in Nurestan Province, Afghanistan.</obo:IAO_0000115>
        <oboInOwl:hasOBONamespace>GAZ</oboInOwl:hasOBONamespace>
        <oboInOwl:id>GAZ:00021703</oboInOwl:id>
        <rdfs:label>Wama District</rdfs:label>
    </owl:NamedIndividual>
    


    <!-- http://purl.obolibrary.org/obo/GAZ_00021704 -->

    <owl:NamedIndividual rdf:about="http://purl.obolibrary.org/obo/GAZ_00021704">
        <rdf:type rdf:resource="http://purl.obolibrary.org/obo/ENVO_00000004"/>
        <obo:RO_0001025 rdf:resource="http://purl.obolibrary.org/obo/GAZ_00010630"/>
        <obo:IAO_0000115>A district in the north of Nangarhar Province, Afghanistan, on the Kunar River.</obo:IAO_0000115>
        <oboInOwl:hasOBONamespace>GAZ</oboInOwl:hasOBONamespace>
        <oboInOwl:id>GAZ:00021704</oboInOwl:id>
        <rdfs:label>Kuz Kunar District</rdfs:label>
    </owl:NamedIndividual>
    


    <!-- http://purl.obolibrary.org/obo/GAZ_00021705 -->

    <owl:NamedIndividual rdf:about="http://purl.obolibrary.org/obo/GAZ_00021705">
        <rdf:type rdf:resource="http://purl.obolibrary.org/obo/ENVO_00000004"/>
        <obo:RO_0001025 rdf:resource="http://purl.obolibrary.org/obo/GAZ_00010626"/>
        <obo:IAO_0000115>A district of Nimruz Province, Afghanistan.</obo:IAO_0000115>
        <oboInOwl:hasOBONamespace>GAZ</oboInOwl:hasOBONamespace>
        <oboInOwl:id>GAZ:00021705</oboInOwl:id>
        <rdfs:label>Chahar Burja District</rdfs:label>
    </owl:NamedIndividual>
    


    <!-- http://purl.obolibrary.org/obo/GAZ_00021706 -->

    <owl:NamedIndividual rdf:about="http://purl.obolibrary.org/obo/GAZ_00021706">
        <rdf:type rdf:resource="http://purl.obolibrary.org/obo/ENVO_00000004"/>
        <obo:RO_0001025 rdf:resource="http://purl.obolibrary.org/obo/GAZ_00010626"/>
        <obo:IAO_0000115>A district of Nimruz Province, Afghanistan.</obo:IAO_0000115>
        <oboInOwl:hasOBONamespace>GAZ</oboInOwl:hasOBONamespace>
        <oboInOwl:id>GAZ:00021706</oboInOwl:id>
        <rdfs:label>Zaranj District</rdfs:label>
    </owl:NamedIndividual>
    


    <!-- http://purl.obolibrary.org/obo/GAZ_00021707 -->

    <owl:NamedIndividual rdf:about="http://purl.obolibrary.org/obo/GAZ_00021707">
        <rdf:type rdf:resource="http://purl.obolibrary.org/obo/ENVO_00000004"/>
        <obo:RO_0001025 rdf:resource="http://purl.obolibrary.org/obo/GAZ_00010631"/>
        <obo:IAO_0000115>A district in Nurestan Province, Afghanistan.</obo:IAO_0000115>
        <oboInOwl:hasOBONamespace>GAZ</oboInOwl:hasOBONamespace>
        <oboInOwl:id>GAZ:00021707</oboInOwl:id>
        <rdfs:label>Kamdesh District</rdfs:label>
    </owl:NamedIndividual>
    


    <!-- http://purl.obolibrary.org/obo/GAZ_00021708 -->

    <owl:NamedIndividual rdf:about="http://purl.obolibrary.org/obo/GAZ_00021708">
        <rdf:type rdf:resource="http://purl.obolibrary.org/obo/ENVO_00000004"/>
        <obo:RO_0001025 rdf:resource="http://purl.obolibrary.org/obo/GAZ_00010630"/>
        <obo:IAO_0000115>A district in the north of Nangarhar Province, Afghanistan. The district contains the provincial capital, Jalalabad.</obo:IAO_0000115>
        <oboInOwl:hasOBONamespace>GAZ</oboInOwl:hasOBONamespace>
        <oboInOwl:id>GAZ:00021708</oboInOwl:id>
        <rdfs:label>Jalalabad District</rdfs:label>
    </owl:NamedIndividual>
    


    <!-- http://purl.obolibrary.org/obo/GAZ_00021709 -->

    <owl:NamedIndividual rdf:about="http://purl.obolibrary.org/obo/GAZ_00021709">
        <rdf:type rdf:resource="http://purl.obolibrary.org/obo/ENVO_00000004"/>
        <obo:RO_0001025 rdf:resource="http://purl.obolibrary.org/obo/GAZ_00010631"/>
        <obo:IAO_0000115>A district in Nurestan Province, Afghanistan.</obo:IAO_0000115>
        <oboInOwl:hasOBONamespace>GAZ</oboInOwl:hasOBONamespace>
        <oboInOwl:id>GAZ:00021709</oboInOwl:id>
        <rdfs:label>Waygal District</rdfs:label>
    </owl:NamedIndividual>
    


    <!-- http://purl.obolibrary.org/obo/GAZ_00021710 -->

    <owl:NamedIndividual rdf:about="http://purl.obolibrary.org/obo/GAZ_00021710">
        <rdf:type rdf:resource="http://purl.obolibrary.org/obo/ENVO_00000004"/>
        <obo:RO_0001025 rdf:resource="http://purl.obolibrary.org/obo/GAZ_00010630"/>
        <obo:IAO_0000115>A district in the west of Nangarhar Province, Afghanistan.</obo:IAO_0000115>
        <oboInOwl:hasOBONamespace>GAZ</oboInOwl:hasOBONamespace>
        <oboInOwl:id>GAZ:00021710</oboInOwl:id>
        <rdfs:label>Hisarak District</rdfs:label>
    </owl:NamedIndividual>
    


    <!-- http://purl.obolibrary.org/obo/GAZ_00021711 -->

    <owl:NamedIndividual rdf:about="http://purl.obolibrary.org/obo/GAZ_00021711">
        <rdf:type rdf:resource="http://purl.obolibrary.org/obo/ENVO_00000004"/>
        <obo:RO_0001025 rdf:resource="http://purl.obolibrary.org/obo/GAZ_00010630"/>
        <obo:IAO_0000115>A district in the south of Nangarhar Province, Afghanistan, bordering on Pakistan.</obo:IAO_0000115>
        <oboInOwl:hasOBONamespace>GAZ</oboInOwl:hasOBONamespace>
        <oboInOwl:id>GAZ:00021711</oboInOwl:id>
        <rdfs:label>Dih Bala District</rdfs:label>
    </owl:NamedIndividual>
    


    <!-- http://purl.obolibrary.org/obo/GAZ_00021712 -->

    <owl:NamedIndividual rdf:about="http://purl.obolibrary.org/obo/GAZ_00021712">
        <rdf:type rdf:resource="http://purl.obolibrary.org/obo/ENVO_00000004"/>
        <obo:RO_0001025 rdf:resource="http://purl.obolibrary.org/obo/GAZ_00010626"/>
        <obo:IAO_0000115>A district of Nimruz Province, Afghanistan.</obo:IAO_0000115>
        <oboInOwl:hasOBONamespace>GAZ</oboInOwl:hasOBONamespace>
        <oboInOwl:id>GAZ:00021712</oboInOwl:id>
        <rdfs:label>Khash Rod District</rdfs:label>
    </owl:NamedIndividual>
    


    <!-- http://purl.obolibrary.org/obo/GAZ_00021713 -->

    <owl:NamedIndividual rdf:about="http://purl.obolibrary.org/obo/GAZ_00021713">
        <rdf:type rdf:resource="http://purl.obolibrary.org/obo/ENVO_00000004"/>
        <obo:RO_0001025 rdf:resource="http://purl.obolibrary.org/obo/GAZ_00010630"/>
        <obo:IAO_0000115>A district in the south of Nangarhar Province, Afghanistan, bordering on Pakistan.</obo:IAO_0000115>
        <oboInOwl:hasOBONamespace>GAZ</oboInOwl:hasOBONamespace>
        <oboInOwl:id>GAZ:00021713</oboInOwl:id>
        <rdfs:label>Khogyani District</rdfs:label>
    </owl:NamedIndividual>
    


    <!-- http://purl.obolibrary.org/obo/GAZ_00021714 -->

    <owl:NamedIndividual rdf:about="http://purl.obolibrary.org/obo/GAZ_00021714">
        <rdf:type rdf:resource="http://purl.obolibrary.org/obo/ENVO_00000004"/>
        <obo:RO_0001025 rdf:resource="http://purl.obolibrary.org/obo/GAZ_00010630"/>
        <obo:IAO_0000115>A district in the southeast of Nangarhar Province, Afghanistan, bordering Pakistan.</obo:IAO_0000115>
        <oboInOwl:hasOBONamespace>GAZ</oboInOwl:hasOBONamespace>
        <oboInOwl:id>GAZ:00021714</oboInOwl:id>
        <rdfs:label>Dur Baba District</rdfs:label>
    </owl:NamedIndividual>
    


    <!-- http://purl.obolibrary.org/obo/GAZ_00021715 -->

    <owl:NamedIndividual rdf:about="http://purl.obolibrary.org/obo/GAZ_00021715">
        <rdf:type rdf:resource="http://purl.obolibrary.org/obo/ENVO_00000004"/>
        <obo:RO_0001025 rdf:resource="http://purl.obolibrary.org/obo/GAZ_00010626"/>
        <obo:IAO_0000115>A district of Nimruz Province, Afghanistan.</obo:IAO_0000115>
        <oboInOwl:hasOBONamespace>GAZ</oboInOwl:hasOBONamespace>
        <oboInOwl:id>GAZ:00021715</oboInOwl:id>
        <rdfs:label>Chakhansur District</rdfs:label>
    </owl:NamedIndividual>
    


    <!-- http://purl.obolibrary.org/obo/GAZ_00021716 -->

    <owl:NamedIndividual rdf:about="http://purl.obolibrary.org/obo/GAZ_00021716">
        <rdf:type rdf:resource="http://purl.obolibrary.org/obo/ENVO_00000004"/>
        <obo:RO_0001025 rdf:resource="http://purl.obolibrary.org/obo/GAZ_00010631"/>
        <obo:IAO_0000115>A district in Nurestan Province, Afghanistan.</obo:IAO_0000115>
        <oboInOwl:hasOBONamespace>GAZ</oboInOwl:hasOBONamespace>
        <oboInOwl:id>GAZ:00021716</oboInOwl:id>
        <rdfs:label>Mandol District</rdfs:label>
    </owl:NamedIndividual>
    


    <!-- http://purl.obolibrary.org/obo/GAZ_00021717 -->

    <owl:NamedIndividual rdf:about="http://purl.obolibrary.org/obo/GAZ_00021717">
        <rdf:type rdf:resource="http://purl.obolibrary.org/obo/ENVO_00000004"/>
        <obo:RO_0001025 rdf:resource="http://purl.obolibrary.org/obo/GAZ_00010630"/>
        <obo:IAO_0000115>A district in Nangarhar Province, Afghanistan, to the east of Jalalabad.</obo:IAO_0000115>
        <oboInOwl:hasOBONamespace>GAZ</oboInOwl:hasOBONamespace>
        <oboInOwl:id>GAZ:00021717</oboInOwl:id>
        <rdfs:label>Kama District</rdfs:label>
    </owl:NamedIndividual>
    


    <!-- http://purl.obolibrary.org/obo/GAZ_00021718 -->

    <owl:NamedIndividual rdf:about="http://purl.obolibrary.org/obo/GAZ_00021718">
        <rdf:type rdf:resource="http://purl.obolibrary.org/obo/ENVO_00000004"/>
        <obo:RO_0001025 rdf:resource="http://purl.obolibrary.org/obo/GAZ_00010630"/>
        <obo:IAO_0000115>A district in the south of Nangarhar Province, Afghanistan, bordering on Pakistan.</obo:IAO_0000115>
        <oboInOwl:hasOBONamespace>GAZ</oboInOwl:hasOBONamespace>
        <oboInOwl:id>GAZ:00021718</oboInOwl:id>
        <rdfs:label>Achin District</rdfs:label>
    </owl:NamedIndividual>
    


    <!-- http://purl.obolibrary.org/obo/GAZ_00021719 -->

    <owl:NamedIndividual rdf:about="http://purl.obolibrary.org/obo/GAZ_00021719">
        <rdf:type rdf:resource="http://purl.obolibrary.org/obo/ENVO_00000004"/>
        <obo:RO_0001025 rdf:resource="http://purl.obolibrary.org/obo/GAZ_00010630"/>
        <obo:IAO_0000115>A district in the northeast of Nangarhar Province, Afghanistan, bordering on Pakistan.</obo:IAO_0000115>
        <oboInOwl:hasOBONamespace>GAZ</oboInOwl:hasOBONamespace>
        <oboInOwl:id>GAZ:00021719</oboInOwl:id>
        <rdfs:label>Goshta District</rdfs:label>
    </owl:NamedIndividual>
    


    <!-- http://purl.obolibrary.org/obo/GAZ_00021720 -->

    <owl:NamedIndividual rdf:about="http://purl.obolibrary.org/obo/GAZ_00021720">
        <rdf:type rdf:resource="http://purl.obolibrary.org/obo/ENVO_00000004"/>
        <obo:RO_0001025 rdf:resource="http://purl.obolibrary.org/obo/GAZ_00010630"/>
        <obo:IAO_0000115>A district in the centre of Nangarhar Province, Afghanistan.</obo:IAO_0000115>
        <oboInOwl:hasOBONamespace>GAZ</oboInOwl:hasOBONamespace>
        <oboInOwl:id>GAZ:00021720</oboInOwl:id>
        <rdfs:label>Chaparhar District</rdfs:label>
    </owl:NamedIndividual>
    


    <!-- http://purl.obolibrary.org/obo/GAZ_00021721 -->

    <owl:NamedIndividual rdf:about="http://purl.obolibrary.org/obo/GAZ_00021721">
        <rdf:type rdf:resource="http://purl.obolibrary.org/obo/ENVO_00000004"/>
        <obo:RO_0001025 rdf:resource="http://purl.obolibrary.org/obo/GAZ_00010630"/>
        <obo:IAO_0000115>A district in the east of Nangarhar Province, Afghanistan.</obo:IAO_0000115>
        <oboInOwl:hasOBONamespace>GAZ</oboInOwl:hasOBONamespace>
        <oboInOwl:id>GAZ:00021721</oboInOwl:id>
        <rdfs:label>Bati Kot District</rdfs:label>
    </owl:NamedIndividual>
    


    <!-- http://purl.obolibrary.org/obo/GAZ_00021722 -->

    <owl:NamedIndividual rdf:about="http://purl.obolibrary.org/obo/GAZ_00021722">
        <rdf:type rdf:resource="http://purl.obolibrary.org/obo/ENVO_00000004"/>
        <obo:RO_0001025 rdf:resource="http://purl.obolibrary.org/obo/GAZ_00010630"/>
        <obo:IAO_0000115>A district in the north of Nangarhar Province, Afghanistan.</obo:IAO_0000115>
        <oboInOwl:hasOBONamespace>GAZ</oboInOwl:hasOBONamespace>
        <oboInOwl:id>GAZ:00021722</oboInOwl:id>
        <rdfs:label>Dara-I-Nur District</rdfs:label>
    </owl:NamedIndividual>
    


    <!-- http://purl.obolibrary.org/obo/GAZ_00021723 -->

    <owl:NamedIndividual rdf:about="http://purl.obolibrary.org/obo/GAZ_00021723">
        <rdf:type rdf:resource="http://purl.obolibrary.org/obo/ENVO_00000004"/>
        <obo:RO_0001025 rdf:resource="http://purl.obolibrary.org/obo/GAZ_00010626"/>
        <obo:IAO_0000115>A district of Nimruz Province, Afghanistan.</obo:IAO_0000115>
        <oboInOwl:hasOBONamespace>GAZ</oboInOwl:hasOBONamespace>
        <oboInOwl:id>GAZ:00021723</oboInOwl:id>
        <rdfs:label>Kang District</rdfs:label>
    </owl:NamedIndividual>
    


    <!-- http://purl.obolibrary.org/obo/GAZ_00021724 -->

    <owl:NamedIndividual rdf:about="http://purl.obolibrary.org/obo/GAZ_00021724">
        <rdf:type rdf:resource="http://purl.obolibrary.org/obo/ENVO_00000004"/>
        <obo:RO_0001025 rdf:resource="http://purl.obolibrary.org/obo/GAZ_00010631"/>
        <obo:IAO_0000115>A district in Nurestan Province, Afghanistan.</obo:IAO_0000115>
        <oboInOwl:hasOBONamespace>GAZ</oboInOwl:hasOBONamespace>
        <oboInOwl:id>GAZ:00021724</oboInOwl:id>
        <rdfs:label>Nurestan District</rdfs:label>
    </owl:NamedIndividual>
    


    <!-- http://purl.obolibrary.org/obo/GAZ_00021725 -->

    <owl:NamedIndividual rdf:about="http://purl.obolibrary.org/obo/GAZ_00021725">
        <rdf:type rdf:resource="http://purl.obolibrary.org/obo/ENVO_00000004"/>
        <obo:RO_0001025 rdf:resource="http://purl.obolibrary.org/obo/GAZ_00010631"/>
        <obo:IAO_0000115>A district in Nurestan Province, Afghanistan.</obo:IAO_0000115>
        <oboInOwl:hasOBONamespace>GAZ</oboInOwl:hasOBONamespace>
        <oboInOwl:id>GAZ:00021725</oboInOwl:id>
        <rdfs:label>Bargi Matal District</rdfs:label>
    </owl:NamedIndividual>
    


    <!-- http://purl.obolibrary.org/obo/GAZ_00021726 -->

    <owl:NamedIndividual rdf:about="http://purl.obolibrary.org/obo/GAZ_00021726">
        <rdf:type rdf:resource="http://purl.obolibrary.org/obo/ENVO_00000004"/>
        <obo:RO_0001025 rdf:resource="http://purl.obolibrary.org/obo/GAZ_00010646"/>
        <obo:IAO_0000115>A district in Paktia Province, Afghanistan.</obo:IAO_0000115>
        <oboInOwl:hasOBONamespace>GAZ</oboInOwl:hasOBONamespace>
        <oboInOwl:id>GAZ:00021726</oboInOwl:id>
        <rdfs:label>Shwak District</rdfs:label>
    </owl:NamedIndividual>
    


    <!-- http://purl.obolibrary.org/obo/GAZ_00021727 -->

    <owl:NamedIndividual rdf:about="http://purl.obolibrary.org/obo/GAZ_00021727">
        <rdf:type rdf:resource="http://purl.obolibrary.org/obo/ENVO_00000004"/>
        <obo:RO_0001025 rdf:resource="http://purl.obolibrary.org/obo/GAZ_00010646"/>
        <obo:IAO_0000115>A district in Paktia Province, Afghanistan.</obo:IAO_0000115>
        <oboInOwl:hasOBONamespace>GAZ</oboInOwl:hasOBONamespace>
        <oboInOwl:id>GAZ:00021727</oboInOwl:id>
        <rdfs:label>Gardez District</rdfs:label>
    </owl:NamedIndividual>
    


    <!-- http://purl.obolibrary.org/obo/GAZ_00021728 -->

    <owl:NamedIndividual rdf:about="http://purl.obolibrary.org/obo/GAZ_00021728">
        <rdf:type rdf:resource="http://purl.obolibrary.org/obo/ENVO_00000004"/>
        <obo:RO_0001025 rdf:resource="http://purl.obolibrary.org/obo/GAZ_00010629"/>
        <obo:IAO_0000115>A district of Oruzgan Province, Afghanistan.</obo:IAO_0000115>
        <oboInOwl:hasOBONamespace>GAZ</oboInOwl:hasOBONamespace>
        <oboInOwl:id>GAZ:00021728</oboInOwl:id>
        <rdfs:label>Tirin Kot District</rdfs:label>
    </owl:NamedIndividual>
    


    <!-- http://purl.obolibrary.org/obo/GAZ_00021729 -->

    <owl:NamedIndividual rdf:about="http://purl.obolibrary.org/obo/GAZ_00021729">
        <rdf:type rdf:resource="http://purl.obolibrary.org/obo/ENVO_00000004"/>
        <obo:RO_0001025 rdf:resource="http://purl.obolibrary.org/obo/GAZ_00010646"/>
        <obo:IAO_0000115>A district in Paktia Province, Afghanistan.</obo:IAO_0000115>
        <oboInOwl:hasOBONamespace>GAZ</oboInOwl:hasOBONamespace>
        <oboInOwl:id>GAZ:00021729</oboInOwl:id>
        <rdfs:label>Jani Khel District</rdfs:label>
    </owl:NamedIndividual>
    


    <!-- http://purl.obolibrary.org/obo/GAZ_00021730 -->

    <owl:NamedIndividual rdf:about="http://purl.obolibrary.org/obo/GAZ_00021730">
        <rdf:type rdf:resource="http://purl.obolibrary.org/obo/ENVO_00000004"/>
        <obo:RO_0001025 rdf:resource="http://purl.obolibrary.org/obo/GAZ_00010646"/>
        <obo:IAO_0000115>A district in Paktia Province, Afghanistan.</obo:IAO_0000115>
        <oboInOwl:hasOBONamespace>GAZ</oboInOwl:hasOBONamespace>
        <oboInOwl:id>GAZ:00021730</oboInOwl:id>
        <rdfs:label>Chamkani District</rdfs:label>
    </owl:NamedIndividual>
    


    <!-- http://purl.obolibrary.org/obo/GAZ_00021732 -->

    <owl:NamedIndividual rdf:about="http://purl.obolibrary.org/obo/GAZ_00021732">
        <rdf:type rdf:resource="http://purl.obolibrary.org/obo/ENVO_00000004"/>
        <obo:RO_0001025 rdf:resource="http://purl.obolibrary.org/obo/GAZ_00010645"/>
        <obo:IAO_0000115>A district of Paktika Province, Afghanistan.</obo:IAO_0000115>
        <oboInOwl:hasOBONamespace>GAZ</oboInOwl:hasOBONamespace>
        <oboInOwl:id>GAZ:00021732</oboInOwl:id>
        <rdfs:label>Zarghun Shahr District</rdfs:label>
    </owl:NamedIndividual>
    


    <!-- http://purl.obolibrary.org/obo/GAZ_00021733 -->

    <owl:NamedIndividual rdf:about="http://purl.obolibrary.org/obo/GAZ_00021733">
        <rdf:type rdf:resource="http://purl.obolibrary.org/obo/ENVO_00000004"/>
        <obo:RO_0001025 rdf:resource="http://purl.obolibrary.org/obo/GAZ_00010646"/>
        <obo:IAO_0000115>A district in Paktia Province, Afghanistan.</obo:IAO_0000115>
        <oboInOwl:hasOBONamespace>GAZ</oboInOwl:hasOBONamespace>
        <oboInOwl:id>GAZ:00021733</oboInOwl:id>
        <rdfs:label>Lija Mangal District</rdfs:label>
    </owl:NamedIndividual>
    


    <!-- http://purl.obolibrary.org/obo/GAZ_00021734 -->

    <owl:NamedIndividual rdf:about="http://purl.obolibrary.org/obo/GAZ_00021734">
        <rdf:type rdf:resource="http://purl.obolibrary.org/obo/ENVO_00000004"/>
        <obo:RO_0001025 rdf:resource="http://purl.obolibrary.org/obo/GAZ_00010646"/>
        <obo:IAO_0000115>A district in Paktia Province, Afghanistan.</obo:IAO_0000115>
        <oboInOwl:hasOBONamespace>GAZ</oboInOwl:hasOBONamespace>
        <oboInOwl:id>GAZ:00021734</oboInOwl:id>
        <rdfs:label>Jadran District</rdfs:label>
    </owl:NamedIndividual>
    


    <!-- http://purl.obolibrary.org/obo/GAZ_00021735 -->

    <owl:NamedIndividual rdf:about="http://purl.obolibrary.org/obo/GAZ_00021735">
        <rdf:type rdf:resource="http://purl.obolibrary.org/obo/ENVO_00000004"/>
        <obo:RO_0001025 rdf:resource="http://purl.obolibrary.org/obo/GAZ_00010646"/>
        <obo:IAO_0000115>A district in Paktia Province, Afghanistan.</obo:IAO_0000115>
        <oboInOwl:hasOBONamespace>GAZ</oboInOwl:hasOBONamespace>
        <oboInOwl:id>GAZ:00021735</oboInOwl:id>
        <rdfs:label>Dand Wa Patan District</rdfs:label>
    </owl:NamedIndividual>
    


    <!-- http://purl.obolibrary.org/obo/GAZ_00021736 -->

    <owl:NamedIndividual rdf:about="http://purl.obolibrary.org/obo/GAZ_00021736">
        <rdf:type rdf:resource="http://purl.obolibrary.org/obo/ENVO_00000004"/>
        <obo:RO_0001025 rdf:resource="http://purl.obolibrary.org/obo/GAZ_00010629"/>
        <obo:IAO_0000115>A district of Oruzgan Province, Afghanistan.</obo:IAO_0000115>
        <oboInOwl:hasOBONamespace>GAZ</oboInOwl:hasOBONamespace>
        <oboInOwl:id>GAZ:00021736</oboInOwl:id>
        <rdfs:label>Khas Uruzgan District</rdfs:label>
    </owl:NamedIndividual>
    


    <!-- http://purl.obolibrary.org/obo/GAZ_00021737 -->

    <owl:NamedIndividual rdf:about="http://purl.obolibrary.org/obo/GAZ_00021737">
        <rdf:type rdf:resource="http://purl.obolibrary.org/obo/ENVO_00000004"/>
        <obo:RO_0001025 rdf:resource="http://purl.obolibrary.org/obo/GAZ_00010646"/>
        <obo:IAO_0000115>A district in Paktia Province, Afghanistan.</obo:IAO_0000115>
        <oboInOwl:hasOBONamespace>GAZ</oboInOwl:hasOBONamespace>
        <oboInOwl:id>GAZ:00021737</oboInOwl:id>
        <rdfs:label>Jaji District</rdfs:label>
    </owl:NamedIndividual>
    


    <!-- http://purl.obolibrary.org/obo/GAZ_00021738 -->

    <owl:NamedIndividual rdf:about="http://purl.obolibrary.org/obo/GAZ_00021738">
        <rdf:type rdf:resource="http://purl.obolibrary.org/obo/ENVO_00000004"/>
        <obo:RO_0001025 rdf:resource="http://purl.obolibrary.org/obo/GAZ_00010629"/>
        <obo:IAO_0000115>A district of Oruzgan Province, Afghanistan.</obo:IAO_0000115>
        <oboInOwl:hasOBONamespace>GAZ</oboInOwl:hasOBONamespace>
        <oboInOwl:id>GAZ:00021738</oboInOwl:id>
        <rdfs:label>Shahidi Hassas District</rdfs:label>
    </owl:NamedIndividual>
    


    <!-- http://purl.obolibrary.org/obo/GAZ_00021739 -->

    <owl:NamedIndividual rdf:about="http://purl.obolibrary.org/obo/GAZ_00021739">
        <rdf:type rdf:resource="http://purl.obolibrary.org/obo/ENVO_00000004"/>
        <obo:RO_0001025 rdf:resource="http://purl.obolibrary.org/obo/GAZ_00010646"/>
        <obo:IAO_0000115>A district in Paktia Province, Afghanistan.</obo:IAO_0000115>
        <oboInOwl:hasOBONamespace>GAZ</oboInOwl:hasOBONamespace>
        <oboInOwl:id>GAZ:00021739</oboInOwl:id>
        <rdfs:label>Zurmat District</rdfs:label>
    </owl:NamedIndividual>
    


    <!-- http://purl.obolibrary.org/obo/GAZ_00021740 -->

    <owl:NamedIndividual rdf:about="http://purl.obolibrary.org/obo/GAZ_00021740">
        <rdf:type rdf:resource="http://purl.obolibrary.org/obo/ENVO_00000004"/>
        <obo:RO_0001025 rdf:resource="http://purl.obolibrary.org/obo/GAZ_00010629"/>
        <obo:IAO_0000115>A district of Oruzgan Province, Afghanistan.</obo:IAO_0000115>
        <oboInOwl:hasOBONamespace>GAZ</oboInOwl:hasOBONamespace>
        <oboInOwl:id>GAZ:00021740</oboInOwl:id>
        <rdfs:label>Chora District</rdfs:label>
    </owl:NamedIndividual>
    


    <!-- http://purl.obolibrary.org/obo/GAZ_00021741 -->

    <owl:NamedIndividual rdf:about="http://purl.obolibrary.org/obo/GAZ_00021741">
        <rdf:type rdf:resource="http://purl.obolibrary.org/obo/ENVO_00000004"/>
        <obo:RO_0001025 rdf:resource="http://purl.obolibrary.org/obo/GAZ_00010629"/>
        <obo:IAO_0000115>A district of Oruzgan Province, Afghanistan.</obo:IAO_0000115>
        <oboInOwl:hasOBONamespace>GAZ</oboInOwl:hasOBONamespace>
        <oboInOwl:id>GAZ:00021741</oboInOwl:id>
        <rdfs:label>Dihrawud District</rdfs:label>
    </owl:NamedIndividual>
    


    <!-- http://purl.obolibrary.org/obo/GAZ_00021742 -->

    <owl:NamedIndividual rdf:about="http://purl.obolibrary.org/obo/GAZ_00021742">
        <obo:RO_0001025 rdf:resource="http://purl.obolibrary.org/obo/GAZ_00010629"/>
        <oboInOwl:hasOBONamespace>GAZ</oboInOwl:hasOBONamespace>
        <oboInOwl:id>GAZ:00021742</oboInOwl:id>
        <rdfs:label>Nesh District</rdfs:label>
    </owl:NamedIndividual>
    


    <!-- http://purl.obolibrary.org/obo/GAZ_00021743 -->

    <owl:NamedIndividual rdf:about="http://purl.obolibrary.org/obo/GAZ_00021743">
        <rdf:type rdf:resource="http://purl.obolibrary.org/obo/ENVO_00000004"/>
        <obo:RO_0001025 rdf:resource="http://purl.obolibrary.org/obo/GAZ_00010646"/>
        <obo:IAO_0000115>A district in Paktia Province, Afghanistan.</obo:IAO_0000115>
        <oboInOwl:hasOBONamespace>GAZ</oboInOwl:hasOBONamespace>
        <oboInOwl:id>GAZ:00021743</oboInOwl:id>
        <rdfs:label>Sayid Karam District</rdfs:label>
    </owl:NamedIndividual>
    


    <!-- http://purl.obolibrary.org/obo/GAZ_00021744 -->

    <owl:NamedIndividual rdf:about="http://purl.obolibrary.org/obo/GAZ_00021744">
        <rdf:type rdf:resource="http://purl.obolibrary.org/obo/ENVO_00000004"/>
        <obo:RO_0001025 rdf:resource="http://purl.obolibrary.org/obo/GAZ_00010646"/>
        <obo:IAO_0000115>A district in Paktia Province, Afghanistan.</obo:IAO_0000115>
        <oboInOwl:hasOBONamespace>GAZ</oboInOwl:hasOBONamespace>
        <oboInOwl:id>GAZ:00021744</oboInOwl:id>
        <rdfs:label>Shamal District</rdfs:label>
    </owl:NamedIndividual>
    


    <!-- http://purl.obolibrary.org/obo/GAZ_00021745 -->

    <owl:NamedIndividual rdf:about="http://purl.obolibrary.org/obo/GAZ_00021745">
        <rdf:type rdf:resource="http://purl.obolibrary.org/obo/ENVO_00000004"/>
        <obo:RO_0001025 rdf:resource="http://purl.obolibrary.org/obo/GAZ_00010640"/>
        <obo:IAO_0000115>A district in the east of Wardak Province, Afghanistan.</obo:IAO_0000115>
        <oboInOwl:hasOBONamespace>GAZ</oboInOwl:hasOBONamespace>
        <oboInOwl:id>GAZ:00021745</oboInOwl:id>
        <rdfs:label>Nirkh District</rdfs:label>
    </owl:NamedIndividual>
    


    <!-- http://purl.obolibrary.org/obo/GAZ_00021746 -->

    <owl:NamedIndividual rdf:about="http://purl.obolibrary.org/obo/GAZ_00021746">
        <rdf:type rdf:resource="http://purl.obolibrary.org/obo/ENVO_00000004"/>
        <obo:RO_0001025 rdf:resource="http://purl.obolibrary.org/obo/GAZ_00010640"/>
        <obo:IAO_0000115>A district of Wardak Province, Afghanistan.</obo:IAO_0000115>
        <oboInOwl:hasOBONamespace>GAZ</oboInOwl:hasOBONamespace>
        <oboInOwl:id>GAZ:00021746</oboInOwl:id>
        <rdfs:label>Saydabad District</rdfs:label>
    </owl:NamedIndividual>
    


    <!-- http://purl.obolibrary.org/obo/GAZ_00021747 -->

    <owl:NamedIndividual rdf:about="http://purl.obolibrary.org/obo/GAZ_00021747">
        <rdf:type rdf:resource="http://purl.obolibrary.org/obo/ENVO_00000004"/>
        <obo:RO_0001025 rdf:resource="http://purl.obolibrary.org/obo/GAZ_00010639"/>
        <obo:IAO_0000115>A district of Zabul Province, Afghanistan.</obo:IAO_0000115>
        <oboInOwl:hasOBONamespace>GAZ</oboInOwl:hasOBONamespace>
        <oboInOwl:id>GAZ:00021747</oboInOwl:id>
        <rdfs:label>Tarnak Wa Jaldak District</rdfs:label>
    </owl:NamedIndividual>
    


    <!-- http://purl.obolibrary.org/obo/GAZ_00021748 -->

    <owl:NamedIndividual rdf:about="http://purl.obolibrary.org/obo/GAZ_00021748">
        <rdf:type rdf:resource="http://purl.obolibrary.org/obo/ENVO_00000004"/>
        <obo:RO_0001025 rdf:resource="http://purl.obolibrary.org/obo/GAZ_00010636"/>
        <obo:IAO_0000115>A district of Sar-e Pol Province, Afghanistan.</obo:IAO_0000115>
        <oboInOwl:hasOBONamespace>GAZ</oboInOwl:hasOBONamespace>
        <oboInOwl:id>GAZ:00021748</oboInOwl:id>
        <rdfs:label>Balkhab District</rdfs:label>
    </owl:NamedIndividual>
    


    <!-- http://purl.obolibrary.org/obo/GAZ_00021749 -->

    <owl:NamedIndividual rdf:about="http://purl.obolibrary.org/obo/GAZ_00021749">
        <rdf:type rdf:resource="http://purl.obolibrary.org/obo/ENVO_00000004"/>
        <obo:RO_0001025 rdf:resource="http://purl.obolibrary.org/obo/GAZ_00010640"/>
        <obo:IAO_0000115>A district of Wardak Province, Afghanistan.</obo:IAO_0000115>
        <oboInOwl:hasOBONamespace>GAZ</oboInOwl:hasOBONamespace>
        <oboInOwl:id>GAZ:00021749</oboInOwl:id>
        <rdfs:label>Markazi Bihsud District</rdfs:label>
    </owl:NamedIndividual>
    


    <!-- http://purl.obolibrary.org/obo/GAZ_00021750 -->

    <owl:NamedIndividual rdf:about="http://purl.obolibrary.org/obo/GAZ_00021750">
        <rdf:type rdf:resource="http://purl.obolibrary.org/obo/ENVO_00000004"/>
        <obo:RO_0001025 rdf:resource="http://purl.obolibrary.org/obo/GAZ_00010639"/>
        <obo:IAO_0000115>A district of Zabul Province, Afghanistan.</obo:IAO_0000115>
        <oboInOwl:hasOBONamespace>GAZ</oboInOwl:hasOBONamespace>
        <oboInOwl:id>GAZ:00021750</oboInOwl:id>
        <rdfs:label>Argahandab District</rdfs:label>
    </owl:NamedIndividual>
    


    <!-- http://purl.obolibrary.org/obo/GAZ_00021751 -->

    <owl:NamedIndividual rdf:about="http://purl.obolibrary.org/obo/GAZ_00021751">
        <rdf:type rdf:resource="http://purl.obolibrary.org/obo/ENVO_00000004"/>
        <obo:RO_0001025 rdf:resource="http://purl.obolibrary.org/obo/GAZ_00010640"/>
        <obo:IAO_0000115>A district of Wardak Province, Afghanistan.</obo:IAO_0000115>
        <oboInOwl:hasOBONamespace>GAZ</oboInOwl:hasOBONamespace>
        <oboInOwl:id>GAZ:00021751</oboInOwl:id>
        <rdfs:label>Day Mirdad District</rdfs:label>
    </owl:NamedIndividual>
    


    <!-- http://purl.obolibrary.org/obo/GAZ_00021752 -->

    <owl:NamedIndividual rdf:about="http://purl.obolibrary.org/obo/GAZ_00021752">
        <rdf:type rdf:resource="http://purl.obolibrary.org/obo/ENVO_00000004"/>
        <obo:RO_0001025 rdf:resource="http://purl.obolibrary.org/obo/GAZ_00010639"/>
        <obo:IAO_0000115>A district of Zabul Province, Afghanistan.</obo:IAO_0000115>
        <oboInOwl:hasOBONamespace>GAZ</oboInOwl:hasOBONamespace>
        <oboInOwl:id>GAZ:00021752</oboInOwl:id>
        <rdfs:label>Atghar District</rdfs:label>
    </owl:NamedIndividual>
    


    <!-- http://purl.obolibrary.org/obo/GAZ_00021753 -->

    <owl:NamedIndividual rdf:about="http://purl.obolibrary.org/obo/GAZ_00021753">
        <rdf:type rdf:resource="http://purl.obolibrary.org/obo/ENVO_00000004"/>
        <obo:RO_0001025 rdf:resource="http://purl.obolibrary.org/obo/GAZ_00010640"/>
        <obo:IAO_0000115>A district in the east of Maydan Shahr, Wardak Province, Afghanistan.</obo:IAO_0000115>
        <oboInOwl:hasOBONamespace>GAZ</oboInOwl:hasOBONamespace>
        <oboInOwl:id>GAZ:00021753</oboInOwl:id>
        <rdfs:label>Jalrez District</rdfs:label>
    </owl:NamedIndividual>
    


    <!-- http://purl.obolibrary.org/obo/GAZ_00021754 -->

    <owl:NamedIndividual rdf:about="http://purl.obolibrary.org/obo/GAZ_00021754">
        <rdf:type rdf:resource="http://purl.obolibrary.org/obo/ENVO_00000004"/>
        <obo:RO_0001025 rdf:resource="http://purl.obolibrary.org/obo/GAZ_00010639"/>
        <obo:IAO_0000115>A district of Zabul Province, Afghanistan.</obo:IAO_0000115>
        <oboInOwl:hasOBONamespace>GAZ</oboInOwl:hasOBONamespace>
        <oboInOwl:id>GAZ:00021754</oboInOwl:id>
        <rdfs:label>Daychopan District</rdfs:label>
    </owl:NamedIndividual>
    


    <!-- http://purl.obolibrary.org/obo/GAZ_00021755 -->

    <owl:NamedIndividual rdf:about="http://purl.obolibrary.org/obo/GAZ_00021755">
        <rdf:type rdf:resource="http://purl.obolibrary.org/obo/ENVO_00000004"/>
        <obo:RO_0001025 rdf:resource="http://purl.obolibrary.org/obo/GAZ_00010640"/>
        <obo:IAO_0000115>A district of Wardak Province, Afghanistan.</obo:IAO_0000115>
        <oboInOwl:hasOBONamespace>GAZ</oboInOwl:hasOBONamespace>
        <oboInOwl:id>GAZ:00021755</oboInOwl:id>
        <rdfs:label>Chak District</rdfs:label>
    </owl:NamedIndividual>
    


    <!-- http://purl.obolibrary.org/obo/GAZ_00021756 -->

    <owl:NamedIndividual rdf:about="http://purl.obolibrary.org/obo/GAZ_00021756">
        <rdf:type rdf:resource="http://purl.obolibrary.org/obo/ENVO_00000004"/>
        <obo:RO_0001025 rdf:resource="http://purl.obolibrary.org/obo/GAZ_00010638"/>
        <obo:IAO_0000115>A district of Takhar Province, Afghanistan.</obo:IAO_0000115>
        <oboInOwl:hasOBONamespace>GAZ</oboInOwl:hasOBONamespace>
        <oboInOwl:id>GAZ:00021756</oboInOwl:id>
        <rdfs:label>Darqad District</rdfs:label>
    </owl:NamedIndividual>
    


    <!-- http://purl.obolibrary.org/obo/GAZ_00021757 -->

    <owl:NamedIndividual rdf:about="http://purl.obolibrary.org/obo/GAZ_00021757">
        <rdf:type rdf:resource="http://purl.obolibrary.org/obo/ENVO_00000004"/>
        <obo:RO_0001025 rdf:resource="http://purl.obolibrary.org/obo/GAZ_00010640"/>
        <obo:IAO_0000115>A district in the east of Wardak Province, Afghanistan.</obo:IAO_0000115>
        <oboInOwl:hasOBONamespace>GAZ</oboInOwl:hasOBONamespace>
        <oboInOwl:id>GAZ:00021757</oboInOwl:id>
        <rdfs:label>Maydan Shahr District</rdfs:label>
    </owl:NamedIndividual>
    


    <!-- http://purl.obolibrary.org/obo/GAZ_00021758 -->

    <owl:NamedIndividual rdf:about="http://purl.obolibrary.org/obo/GAZ_00021758">
        <rdf:type rdf:resource="http://purl.obolibrary.org/obo/ENVO_00000004"/>
        <obo:RO_0001025 rdf:resource="http://purl.obolibrary.org/obo/GAZ_00010639"/>
        <obo:IAO_0000115>A district of Zabul Province, Afghanistan.</obo:IAO_0000115>
        <oboInOwl:hasOBONamespace>GAZ</oboInOwl:hasOBONamespace>
        <oboInOwl:id>GAZ:00021758</oboInOwl:id>
        <rdfs:label>Shinkay District</rdfs:label>
    </owl:NamedIndividual>
    


    <!-- http://purl.obolibrary.org/obo/GAZ_00021759 -->

    <owl:NamedIndividual rdf:about="http://purl.obolibrary.org/obo/GAZ_00021759">
        <rdf:type rdf:resource="http://purl.obolibrary.org/obo/ENVO_00000004"/>
        <obo:RO_0001025 rdf:resource="http://purl.obolibrary.org/obo/GAZ_00010639"/>
        <obo:IAO_0000115>A district of Zabul Province, Afghanistan.</obo:IAO_0000115>
        <oboInOwl:hasOBONamespace>GAZ</oboInOwl:hasOBONamespace>
        <oboInOwl:id>GAZ:00021759</oboInOwl:id>
        <rdfs:label>Qalat District</rdfs:label>
    </owl:NamedIndividual>
    


    <!-- http://purl.obolibrary.org/obo/GAZ_00021760 -->

    <owl:NamedIndividual rdf:about="http://purl.obolibrary.org/obo/GAZ_00021760">
        <rdf:type rdf:resource="http://purl.obolibrary.org/obo/ENVO_00000004"/>
        <obo:RO_0001025 rdf:resource="http://purl.obolibrary.org/obo/GAZ_00010639"/>
        <obo:IAO_0000115>A district of Zabul Province, Afghanistan.</obo:IAO_0000115>
        <oboInOwl:hasOBONamespace>GAZ</oboInOwl:hasOBONamespace>
        <oboInOwl:id>GAZ:00021760</oboInOwl:id>
        <rdfs:label>Shahjoy District</rdfs:label>
    </owl:NamedIndividual>
    


    <!-- http://purl.obolibrary.org/obo/GAZ_00021761 -->

    <owl:NamedIndividual rdf:about="http://purl.obolibrary.org/obo/GAZ_00021761">
        <rdf:type rdf:resource="http://purl.obolibrary.org/obo/ENVO_00000004"/>
        <obo:RO_0001025 rdf:resource="http://purl.obolibrary.org/obo/GAZ_00010640"/>
        <obo:IAO_0000115>A district of Wardak Province, Afghanistan.</obo:IAO_0000115>
        <oboInOwl:hasOBONamespace>GAZ</oboInOwl:hasOBONamespace>
        <oboInOwl:id>GAZ:00021761</oboInOwl:id>
        <rdfs:label>Hisa-I-Awal Bihsud District</rdfs:label>
    </owl:NamedIndividual>
    


    <!-- http://purl.obolibrary.org/obo/GAZ_00021762 -->

    <owl:NamedIndividual rdf:about="http://purl.obolibrary.org/obo/GAZ_00021762">
        <rdf:type rdf:resource="http://purl.obolibrary.org/obo/ENVO_00000004"/>
        <obo:RO_0001025 rdf:resource="http://purl.obolibrary.org/obo/GAZ_00010639"/>
        <obo:IAO_0000115>A district of Zabul Province, Afghanistan.</obo:IAO_0000115>
        <oboInOwl:hasOBONamespace>GAZ</oboInOwl:hasOBONamespace>
        <oboInOwl:id>GAZ:00021762</oboInOwl:id>
        <rdfs:label>Mizan District</rdfs:label>
    </owl:NamedIndividual>
    


    <!-- http://purl.obolibrary.org/obo/GAZ_00021763 -->

    <owl:NamedIndividual rdf:about="http://purl.obolibrary.org/obo/GAZ_00021763">
        <rdf:type rdf:resource="http://purl.obolibrary.org/obo/ENVO_00000004"/>
        <obo:RO_0001025 rdf:resource="http://purl.obolibrary.org/obo/GAZ_00010639"/>
        <obo:IAO_0000115>A district of Zabul Province, Afghanistan.</obo:IAO_0000115>
        <oboInOwl:hasOBONamespace>GAZ</oboInOwl:hasOBONamespace>
        <oboInOwl:id>GAZ:00021763</oboInOwl:id>
        <rdfs:label>Shamulzayi District</rdfs:label>
    </owl:NamedIndividual>
    


    <!-- http://purl.obolibrary.org/obo/GAZ_00021764 -->

    <owl:NamedIndividual rdf:about="http://purl.obolibrary.org/obo/GAZ_00021764">
        <rdf:type rdf:resource="http://purl.obolibrary.org/obo/ENVO_00000004"/>
        <obo:RO_0001025 rdf:resource="http://purl.obolibrary.org/obo/GAZ_00010647"/>
        <obo:IAO_0000115>A district in Samangan Province, northern Afghanistan.</obo:IAO_0000115>
        <oboInOwl:hasOBONamespace>GAZ</oboInOwl:hasOBONamespace>
        <oboInOwl:id>GAZ:00021764</oboInOwl:id>
        <rdfs:label>Aybak District</rdfs:label>
    </owl:NamedIndividual>
    


    <!-- http://purl.obolibrary.org/obo/GAZ_00021765 -->

    <owl:NamedIndividual rdf:about="http://purl.obolibrary.org/obo/GAZ_00021765">
        <rdf:type rdf:resource="http://purl.obolibrary.org/obo/ENVO_00000004"/>
        <obo:RO_0001025 rdf:resource="http://purl.obolibrary.org/obo/GAZ_00010638"/>
        <obo:IAO_0000115>A district of Takhar Province, Afghanistan.</obo:IAO_0000115>
        <oboInOwl:hasOBONamespace>GAZ</oboInOwl:hasOBONamespace>
        <oboInOwl:id>GAZ:00021765</oboInOwl:id>
        <rdfs:label>Farkhar District</rdfs:label>
    </owl:NamedIndividual>
    


    <!-- http://purl.obolibrary.org/obo/GAZ_00021766 -->

    <owl:NamedIndividual rdf:about="http://purl.obolibrary.org/obo/GAZ_00021766">
        <rdf:type rdf:resource="http://purl.obolibrary.org/obo/ENVO_00000004"/>
        <obo:RO_0001025 rdf:resource="http://purl.obolibrary.org/obo/GAZ_00010638"/>
        <obo:IAO_0000115>A district of Takhar Province, Afghanistan.</obo:IAO_0000115>
        <oboInOwl:hasOBONamespace>GAZ</oboInOwl:hasOBONamespace>
        <oboInOwl:id>GAZ:00021766</oboInOwl:id>
        <rdfs:label>Chah Ab District</rdfs:label>
    </owl:NamedIndividual>
    


    <!-- http://purl.obolibrary.org/obo/GAZ_00021767 -->

    <owl:NamedIndividual rdf:about="http://purl.obolibrary.org/obo/GAZ_00021767">
        <rdf:type rdf:resource="http://purl.obolibrary.org/obo/ENVO_00000004"/>
        <obo:RO_0001025 rdf:resource="http://purl.obolibrary.org/obo/GAZ_00010638"/>
        <obo:IAO_0000115>A district of Takhar Province, Afghanistan.</obo:IAO_0000115>
        <oboInOwl:hasOBONamespace>GAZ</oboInOwl:hasOBONamespace>
        <oboInOwl:id>GAZ:00021767</oboInOwl:id>
        <rdfs:label>Ishkamish District</rdfs:label>
    </owl:NamedIndividual>
    


    <!-- http://purl.obolibrary.org/obo/GAZ_00021768 -->

    <owl:NamedIndividual rdf:about="http://purl.obolibrary.org/obo/GAZ_00021768">
        <rdf:type rdf:resource="http://purl.obolibrary.org/obo/ENVO_00000004"/>
        <obo:RO_0001025 rdf:resource="http://purl.obolibrary.org/obo/GAZ_00010638"/>
        <obo:IAO_0000115>A district of Takhar Province, Afghanistan.</obo:IAO_0000115>
        <oboInOwl:hasOBONamespace>GAZ</oboInOwl:hasOBONamespace>
        <oboInOwl:id>GAZ:00021768</oboInOwl:id>
        <rdfs:label>Yangi Qala District</rdfs:label>
    </owl:NamedIndividual>
    


    <!-- http://purl.obolibrary.org/obo/GAZ_00021769 -->

    <owl:NamedIndividual rdf:about="http://purl.obolibrary.org/obo/GAZ_00021769">
        <rdf:type rdf:resource="http://purl.obolibrary.org/obo/ENVO_00000004"/>
        <obo:RO_0001025 rdf:resource="http://purl.obolibrary.org/obo/GAZ_00010638"/>
        <obo:IAO_0000115>A district of Takhar Province, Afghanistan.</obo:IAO_0000115>
        <oboInOwl:hasOBONamespace>GAZ</oboInOwl:hasOBONamespace>
        <oboInOwl:id>GAZ:00021769</oboInOwl:id>
        <rdfs:label>Chal District</rdfs:label>
    </owl:NamedIndividual>
    


    <!-- http://purl.obolibrary.org/obo/GAZ_00021770 -->

    <owl:NamedIndividual rdf:about="http://purl.obolibrary.org/obo/GAZ_00021770">
        <rdf:type rdf:resource="http://purl.obolibrary.org/obo/ENVO_00000004"/>
        <obo:RO_0001025 rdf:resource="http://purl.obolibrary.org/obo/GAZ_00010638"/>
        <obo:IAO_0000115>A district of Takhar Province, Afghanistan.</obo:IAO_0000115>
        <oboInOwl:hasOBONamespace>GAZ</oboInOwl:hasOBONamespace>
        <oboInOwl:id>GAZ:00021770</oboInOwl:id>
        <rdfs:label>Taluqan District</rdfs:label>
    </owl:NamedIndividual>
    


    <!-- http://purl.obolibrary.org/obo/GAZ_00021771 -->

    <owl:NamedIndividual rdf:about="http://purl.obolibrary.org/obo/GAZ_00021771">
        <rdf:type rdf:resource="http://purl.obolibrary.org/obo/ENVO_00000004"/>
        <obo:RO_0001025 rdf:resource="http://purl.obolibrary.org/obo/GAZ_00010638"/>
        <obo:IAO_0000115>A district of Takhar Province, Afghanistan.</obo:IAO_0000115>
        <oboInOwl:hasOBONamespace>GAZ</oboInOwl:hasOBONamespace>
        <oboInOwl:id>GAZ:00021771</oboInOwl:id>
        <rdfs:label>Kalafgan District</rdfs:label>
    </owl:NamedIndividual>
    


    <!-- http://purl.obolibrary.org/obo/GAZ_00021772 -->

    <owl:NamedIndividual rdf:about="http://purl.obolibrary.org/obo/GAZ_00021772">
        <rdf:type rdf:resource="http://purl.obolibrary.org/obo/ENVO_00000004"/>
        <obo:RO_0001025 rdf:resource="http://purl.obolibrary.org/obo/GAZ_00010638"/>
        <obo:IAO_0000115>A district of Takhar Province, Afghanistan.</obo:IAO_0000115>
        <oboInOwl:hasOBONamespace>GAZ</oboInOwl:hasOBONamespace>
        <oboInOwl:id>GAZ:00021772</oboInOwl:id>
        <rdfs:label>Rustaq District</rdfs:label>
    </owl:NamedIndividual>
    


    <!-- http://purl.obolibrary.org/obo/GAZ_00021773 -->

    <owl:NamedIndividual rdf:about="http://purl.obolibrary.org/obo/GAZ_00021773">
        <rdf:type rdf:resource="http://purl.obolibrary.org/obo/ENVO_00000004"/>
        <obo:RO_0001025 rdf:resource="http://purl.obolibrary.org/obo/GAZ_00010636"/>
        <obo:IAO_0000115>A district of Sar-e Pol Province, Afghanistan.</obo:IAO_0000115>
        <oboInOwl:hasOBONamespace>GAZ</oboInOwl:hasOBONamespace>
        <oboInOwl:id>GAZ:00021773</oboInOwl:id>
        <rdfs:label>Sozma Qala District</rdfs:label>
    </owl:NamedIndividual>
    


    <!-- http://purl.obolibrary.org/obo/GAZ_00021774 -->

    <owl:NamedIndividual rdf:about="http://purl.obolibrary.org/obo/GAZ_00021774">
        <rdf:type rdf:resource="http://purl.obolibrary.org/obo/ENVO_00000004"/>
        <obo:RO_0001025 rdf:resource="http://purl.obolibrary.org/obo/GAZ_00010638"/>
        <obo:IAO_0000115>A district of Takhar Province, Afghanistan.</obo:IAO_0000115>
        <oboInOwl:hasOBONamespace>GAZ</oboInOwl:hasOBONamespace>
        <oboInOwl:id>GAZ:00021774</oboInOwl:id>
        <rdfs:label>Warsaj District</rdfs:label>
    </owl:NamedIndividual>
    


    <!-- http://purl.obolibrary.org/obo/GAZ_00021775 -->

    <owl:NamedIndividual rdf:about="http://purl.obolibrary.org/obo/GAZ_00021775">
        <rdf:type rdf:resource="http://purl.obolibrary.org/obo/ENVO_00000004"/>
        <obo:RO_0001025 rdf:resource="http://purl.obolibrary.org/obo/GAZ_00010647"/>
        <obo:IAO_0000115>A district in Samangan Province, northern Afghanistan.</obo:IAO_0000115>
        <oboInOwl:hasOBONamespace>GAZ</oboInOwl:hasOBONamespace>
        <oboInOwl:id>GAZ:00021775</oboInOwl:id>
        <rdfs:label>Ruyi Du Ab District</rdfs:label>
    </owl:NamedIndividual>
    


    <!-- http://purl.obolibrary.org/obo/GAZ_00021776 -->

    <owl:NamedIndividual rdf:about="http://purl.obolibrary.org/obo/GAZ_00021776">
        <rdf:type rdf:resource="http://purl.obolibrary.org/obo/ENVO_00000004"/>
        <obo:RO_0001025 rdf:resource="http://purl.obolibrary.org/obo/GAZ_00010638"/>
        <obo:IAO_0000115>A district of Takhar Province, Afghanistan.</obo:IAO_0000115>
        <oboInOwl:hasOBONamespace>GAZ</oboInOwl:hasOBONamespace>
        <oboInOwl:id>GAZ:00021776</oboInOwl:id>
        <rdfs:label>Khwaja Ghar District</rdfs:label>
    </owl:NamedIndividual>
    


    <!-- http://purl.obolibrary.org/obo/GAZ_00021777 -->

    <owl:NamedIndividual rdf:about="http://purl.obolibrary.org/obo/GAZ_00021777">
        <rdf:type rdf:resource="http://purl.obolibrary.org/obo/ENVO_00000004"/>
        <obo:RO_0001025 rdf:resource="http://purl.obolibrary.org/obo/GAZ_00010636"/>
        <obo:IAO_0000115>A district of Sar-e Pol Province, Afghanistan.</obo:IAO_0000115>
        <oboInOwl:hasOBONamespace>GAZ</oboInOwl:hasOBONamespace>
        <oboInOwl:id>GAZ:00021777</oboInOwl:id>
        <rdfs:label>Sayyad District</rdfs:label>
    </owl:NamedIndividual>
    


    <!-- http://purl.obolibrary.org/obo/GAZ_00021778 -->

    <owl:NamedIndividual rdf:about="http://purl.obolibrary.org/obo/GAZ_00021778">
        <rdf:type rdf:resource="http://purl.obolibrary.org/obo/ENVO_00000004"/>
        <obo:RO_0001025 rdf:resource="http://purl.obolibrary.org/obo/GAZ_00010636"/>
        <obo:IAO_0000115>A district of Sar-e Pol Province, Afghanistan.</obo:IAO_0000115>
        <oboInOwl:hasOBONamespace>GAZ</oboInOwl:hasOBONamespace>
        <oboInOwl:id>GAZ:00021778</oboInOwl:id>
        <rdfs:label>Sangcharak District</rdfs:label>
    </owl:NamedIndividual>
    


    <!-- http://purl.obolibrary.org/obo/GAZ_00021779 -->

    <owl:NamedIndividual rdf:about="http://purl.obolibrary.org/obo/GAZ_00021779">
        <rdf:type rdf:resource="http://purl.obolibrary.org/obo/ENVO_00000004"/>
        <obo:RO_0001025 rdf:resource="http://purl.obolibrary.org/obo/GAZ_00010638"/>
        <obo:IAO_0000115>A district of Takhar Province, Afghanistan.</obo:IAO_0000115>
        <oboInOwl:hasOBONamespace>GAZ</oboInOwl:hasOBONamespace>
        <oboInOwl:id>GAZ:00021779</oboInOwl:id>
        <rdfs:label>Bangi District</rdfs:label>
    </owl:NamedIndividual>
    


    <!-- http://purl.obolibrary.org/obo/GAZ_00021780 -->

    <owl:NamedIndividual rdf:about="http://purl.obolibrary.org/obo/GAZ_00021780">
        <rdf:type rdf:resource="http://purl.obolibrary.org/obo/ENVO_00000004"/>
        <obo:RO_0001025 rdf:resource="http://purl.obolibrary.org/obo/GAZ_00010647"/>
        <obo:IAO_0000115>A district in Samangan Province, northern Afghanistan.</obo:IAO_0000115>
        <oboInOwl:hasOBONamespace>GAZ</oboInOwl:hasOBONamespace>
        <oboInOwl:id>GAZ:00021780</oboInOwl:id>
        <rdfs:label>Khuram Wa Sarbagh District</rdfs:label>
    </owl:NamedIndividual>
    


    <!-- http://purl.obolibrary.org/obo/GAZ_00021781 -->

    <owl:NamedIndividual rdf:about="http://purl.obolibrary.org/obo/GAZ_00021781">
        <rdf:type rdf:resource="http://purl.obolibrary.org/obo/ENVO_00000004"/>
        <obo:RO_0001025 rdf:resource="http://purl.obolibrary.org/obo/GAZ_00010636"/>
        <obo:IAO_0000115>A district of Sar-e Pol Province, Afghanistan.</obo:IAO_0000115>
        <oboInOwl:hasOBONamespace>GAZ</oboInOwl:hasOBONamespace>
        <oboInOwl:id>GAZ:00021781</oboInOwl:id>
        <rdfs:label>Sare Pol District</rdfs:label>
    </owl:NamedIndividual>
    


    <!-- http://purl.obolibrary.org/obo/GAZ_00021782 -->

    <owl:NamedIndividual rdf:about="http://purl.obolibrary.org/obo/GAZ_00021782">
        <rdf:type rdf:resource="http://purl.obolibrary.org/obo/ENVO_00000004"/>
        <obo:RO_0001025 rdf:resource="http://purl.obolibrary.org/obo/GAZ_00010647"/>
        <obo:IAO_0000115>A district in Samangan Province, northern Afghanistan.</obo:IAO_0000115>
        <oboInOwl:hasOBONamespace>GAZ</oboInOwl:hasOBONamespace>
        <oboInOwl:id>GAZ:00021782</oboInOwl:id>
        <rdfs:label>Dara-I-Suf District</rdfs:label>
    </owl:NamedIndividual>
    


    <!-- http://purl.obolibrary.org/obo/GAZ_00021783 -->

    <owl:NamedIndividual rdf:about="http://purl.obolibrary.org/obo/GAZ_00021783">
        <rdf:type rdf:resource="http://purl.obolibrary.org/obo/ENVO_00000004"/>
        <obo:RO_0001025 rdf:resource="http://purl.obolibrary.org/obo/GAZ_00010636"/>
        <obo:IAO_0000115>A district of Sar-e Pol Province, Afghanistan.</obo:IAO_0000115>
        <oboInOwl:hasOBONamespace>GAZ</oboInOwl:hasOBONamespace>
        <oboInOwl:id>GAZ:00021783</oboInOwl:id>
        <rdfs:label>Kohistanat District</rdfs:label>
    </owl:NamedIndividual>
    


    <!-- http://purl.obolibrary.org/obo/GAZ_00021784 -->

    <owl:NamedIndividual rdf:about="http://purl.obolibrary.org/obo/GAZ_00021784">
        <rdf:type rdf:resource="http://purl.obolibrary.org/obo/ENVO_00000004"/>
        <obo:RO_0001025 rdf:resource="http://purl.obolibrary.org/obo/GAZ_00010647"/>
        <obo:IAO_0000115>A district in Samangan Province, northern Afghanistan.</obo:IAO_0000115>
        <oboInOwl:hasOBONamespace>GAZ</oboInOwl:hasOBONamespace>
        <oboInOwl:id>GAZ:00021784</oboInOwl:id>
        <rdfs:label>Hazrati Sultan District</rdfs:label>
    </owl:NamedIndividual>
    


    <!-- http://purl.obolibrary.org/obo/GAZ_00021785 -->

    <owl:NamedIndividual rdf:about="http://purl.obolibrary.org/obo/GAZ_00021785">
        <rdf:type rdf:resource="http://purl.obolibrary.org/obo/ENVO_00000004"/>
        <obo:RO_0001025 rdf:resource="http://purl.obolibrary.org/obo/GAZ_00010645"/>
        <obo:IAO_0000115>A district of Paktika Province, Afghanistan.</obo:IAO_0000115>
        <oboInOwl:hasOBONamespace>GAZ</oboInOwl:hasOBONamespace>
        <oboInOwl:id>GAZ:00021785</oboInOwl:id>
        <rdfs:label>Ziruk District</rdfs:label>
    </owl:NamedIndividual>
    


    <!-- http://purl.obolibrary.org/obo/GAZ_00021786 -->

    <owl:NamedIndividual rdf:about="http://purl.obolibrary.org/obo/GAZ_00021786">
        <rdf:type rdf:resource="http://purl.obolibrary.org/obo/ENVO_00000004"/>
        <obo:RO_0001025 rdf:resource="http://purl.obolibrary.org/obo/GAZ_00010643"/>
        <obo:IAO_0000115>A district in Panjshir Province, Afghanistan.</obo:IAO_0000115>
        <oboInOwl:hasOBONamespace>GAZ</oboInOwl:hasOBONamespace>
        <oboInOwl:id>GAZ:00021786</oboInOwl:id>
        <rdfs:label>Shootul District</rdfs:label>
    </owl:NamedIndividual>
    


    <!-- http://purl.obolibrary.org/obo/GAZ_00021787 -->

    <owl:NamedIndividual rdf:about="http://purl.obolibrary.org/obo/GAZ_00021787">
        <rdf:type rdf:resource="http://purl.obolibrary.org/obo/ENVO_00000004"/>
        <obo:RO_0001025 rdf:resource="http://purl.obolibrary.org/obo/GAZ_00010644"/>
        <obo:IAO_0000115>A district in Parvan Province, Afghanistan.</obo:IAO_0000115>
        <oboInOwl:hasOBONamespace>GAZ</oboInOwl:hasOBONamespace>
        <oboInOwl:id>GAZ:00021787</oboInOwl:id>
        <rdfs:label>Surkhi Parsa District</rdfs:label>
    </owl:NamedIndividual>
    


    <!-- http://purl.obolibrary.org/obo/GAZ_00021788 -->

    <owl:NamedIndividual rdf:about="http://purl.obolibrary.org/obo/GAZ_00021788">
        <rdf:type rdf:resource="http://purl.obolibrary.org/obo/ENVO_00000004"/>
        <obo:RO_0001025 rdf:resource="http://purl.obolibrary.org/obo/GAZ_00010644"/>
        <obo:IAO_0000115>A district in Parvan Province, Afghanistan.</obo:IAO_0000115>
        <oboInOwl:hasOBONamespace>GAZ</oboInOwl:hasOBONamespace>
        <oboInOwl:id>GAZ:00021788</oboInOwl:id>
        <rdfs:label>Bagram District</rdfs:label>
    </owl:NamedIndividual>
    


    <!-- http://purl.obolibrary.org/obo/GAZ_00021789 -->

    <owl:NamedIndividual rdf:about="http://purl.obolibrary.org/obo/GAZ_00021789">
        <rdf:type rdf:resource="http://purl.obolibrary.org/obo/ENVO_00000004"/>
        <obo:RO_0001025 rdf:resource="http://purl.obolibrary.org/obo/GAZ_00010643"/>
        <obo:IAO_0000115>A district in Panjshir Province, Afghanistan.</obo:IAO_0000115>
        <oboInOwl:hasOBONamespace>GAZ</oboInOwl:hasOBONamespace>
        <oboInOwl:id>GAZ:00021789</oboInOwl:id>
        <rdfs:label>Anaba District</rdfs:label>
    </owl:NamedIndividual>
    


    <!-- http://purl.obolibrary.org/obo/GAZ_00021790 -->

    <owl:NamedIndividual rdf:about="http://purl.obolibrary.org/obo/GAZ_00021790">
        <rdf:type rdf:resource="http://purl.obolibrary.org/obo/ENVO_00000004"/>
        <obo:RO_0001025 rdf:resource="http://purl.obolibrary.org/obo/GAZ_00010644"/>
        <obo:IAO_0000115>A district in Parvan Province, Afghanistan.</obo:IAO_0000115>
        <oboInOwl:hasOBONamespace>GAZ</oboInOwl:hasOBONamespace>
        <oboInOwl:id>GAZ:00021790</oboInOwl:id>
        <rdfs:label>Chaharikar District</rdfs:label>
    </owl:NamedIndividual>
    


    <!-- http://purl.obolibrary.org/obo/GAZ_00021791 -->

    <owl:NamedIndividual rdf:about="http://purl.obolibrary.org/obo/GAZ_00021791">
        <rdf:type rdf:resource="http://purl.obolibrary.org/obo/ENVO_00000004"/>
        <obo:RO_0001025 rdf:resource="http://purl.obolibrary.org/obo/GAZ_00010643"/>
        <obo:IAO_0000115>A district in Panjshir Province, Afghanistan.</obo:IAO_0000115>
        <oboInOwl:hasOBONamespace>GAZ</oboInOwl:hasOBONamespace>
        <oboInOwl:id>GAZ:00021791</oboInOwl:id>
        <rdfs:label>Hisa-I-Awali Panjsher District</rdfs:label>
    </owl:NamedIndividual>
    


    <!-- http://purl.obolibrary.org/obo/GAZ_00021792 -->

    <owl:NamedIndividual rdf:about="http://purl.obolibrary.org/obo/GAZ_00021792">
        <rdf:type rdf:resource="http://purl.obolibrary.org/obo/ENVO_00000004"/>
        <obo:RO_0001025 rdf:resource="http://purl.obolibrary.org/obo/GAZ_00010644"/>
        <obo:IAO_0000115>A district in Parvan Province, Afghanistan.</obo:IAO_0000115>
        <oboInOwl:hasOBONamespace>GAZ</oboInOwl:hasOBONamespace>
        <oboInOwl:id>GAZ:00021792</oboInOwl:id>
        <rdfs:label>Ghorband District</rdfs:label>
    </owl:NamedIndividual>
    


    <!-- http://purl.obolibrary.org/obo/GAZ_00021793 -->

    <owl:NamedIndividual rdf:about="http://purl.obolibrary.org/obo/GAZ_00021793">
        <rdf:type rdf:resource="http://purl.obolibrary.org/obo/ENVO_00000004"/>
        <obo:RO_0001025 rdf:resource="http://purl.obolibrary.org/obo/GAZ_00010644"/>
        <obo:IAO_0000115>A district in Parvan Province, Afghanistan.</obo:IAO_0000115>
        <oboInOwl:hasOBONamespace>GAZ</oboInOwl:hasOBONamespace>
        <oboInOwl:id>GAZ:00021793</oboInOwl:id>
        <rdfs:label>Shekh Ali District</rdfs:label>
    </owl:NamedIndividual>
    


    <!-- http://purl.obolibrary.org/obo/GAZ_00021794 -->

    <owl:NamedIndividual rdf:about="http://purl.obolibrary.org/obo/GAZ_00021794">
        <rdf:type rdf:resource="http://purl.obolibrary.org/obo/ENVO_00000004"/>
        <obo:RO_0001025 rdf:resource="http://purl.obolibrary.org/obo/GAZ_00010643"/>
        <obo:IAO_0000115>A district in Panjshir Province, Afghanistan.</obo:IAO_0000115>
        <oboInOwl:hasOBONamespace>GAZ</oboInOwl:hasOBONamespace>
        <oboInOwl:id>GAZ:00021794</oboInOwl:id>
        <rdfs:label>Rokha District</rdfs:label>
    </owl:NamedIndividual>
    


    <!-- http://purl.obolibrary.org/obo/GAZ_00021795 -->

    <owl:NamedIndividual rdf:about="http://purl.obolibrary.org/obo/GAZ_00021795">
        <rdf:type rdf:resource="http://purl.obolibrary.org/obo/ENVO_00000004"/>
        <obo:RO_0001025 rdf:resource="http://purl.obolibrary.org/obo/GAZ_00010644"/>
        <obo:IAO_0000115>A district in Parvan Province, Afghanistan.</obo:IAO_0000115>
        <oboInOwl:hasOBONamespace>GAZ</oboInOwl:hasOBONamespace>
        <oboInOwl:id>GAZ:00021795</oboInOwl:id>
        <rdfs:label>Kohi Safi District</rdfs:label>
    </owl:NamedIndividual>
    


    <!-- http://purl.obolibrary.org/obo/GAZ_00021796 -->

    <owl:NamedIndividual rdf:about="http://purl.obolibrary.org/obo/GAZ_00021796">
        <rdf:type rdf:resource="http://purl.obolibrary.org/obo/ENVO_00000004"/>
        <obo:RO_0001025 rdf:resource="http://purl.obolibrary.org/obo/GAZ_00010644"/>
        <obo:IAO_0000115>A district of Parwan province located north of the capital Kabul, Afghanistan.</obo:IAO_0000115>
        <oboInOwl:hasOBONamespace>GAZ</oboInOwl:hasOBONamespace>
        <oboInOwl:id>GAZ:00021796</oboInOwl:id>
        <rdfs:label>Jabul Saraj District</rdfs:label>
    </owl:NamedIndividual>
    


    <!-- http://purl.obolibrary.org/obo/GAZ_00021797 -->

    <owl:NamedIndividual rdf:about="http://purl.obolibrary.org/obo/GAZ_00021797">
        <rdf:type rdf:resource="http://purl.obolibrary.org/obo/ENVO_00000004"/>
        <obo:RO_0001025 rdf:resource="http://purl.obolibrary.org/obo/GAZ_00010644"/>
        <obo:IAO_0000115>A district in Parvan Province, Afghanistan.</obo:IAO_0000115>
        <oboInOwl:hasOBONamespace>GAZ</oboInOwl:hasOBONamespace>
        <oboInOwl:id>GAZ:00021797</oboInOwl:id>
        <rdfs:label>Shinwari District</rdfs:label>
    </owl:NamedIndividual>
    


    <!-- http://purl.obolibrary.org/obo/GAZ_00021798 -->

    <owl:NamedIndividual rdf:about="http://purl.obolibrary.org/obo/GAZ_00021798">
        <rdf:type rdf:resource="http://purl.obolibrary.org/obo/ENVO_00000004"/>
        <obo:RO_0001025 rdf:resource="http://purl.obolibrary.org/obo/GAZ_00010645"/>
        <obo:IAO_0000115>A district of Paktika Province, Afghanistan.</obo:IAO_0000115>
        <oboInOwl:hasOBONamespace>GAZ</oboInOwl:hasOBONamespace>
        <oboInOwl:id>GAZ:00021798</oboInOwl:id>
        <rdfs:label>Wor Mamay District</rdfs:label>
    </owl:NamedIndividual>
    


    <!-- http://purl.obolibrary.org/obo/GAZ_00021799 -->

    <owl:NamedIndividual rdf:about="http://purl.obolibrary.org/obo/GAZ_00021799">
        <rdf:type rdf:resource="http://purl.obolibrary.org/obo/ENVO_00000004"/>
        <obo:RO_0001025 rdf:resource="http://purl.obolibrary.org/obo/GAZ_00010643"/>
        <obo:IAO_0000115>A district in Panjshir Province, Afghanistan.</obo:IAO_0000115>
        <oboInOwl:hasOBONamespace>GAZ</oboInOwl:hasOBONamespace>
        <oboInOwl:id>GAZ:00021799</oboInOwl:id>
        <rdfs:label>Hisa-I-Dowom Panjsher District</rdfs:label>
    </owl:NamedIndividual>
    


    <!-- http://purl.obolibrary.org/obo/GAZ_00021800 -->

    <owl:NamedIndividual rdf:about="http://purl.obolibrary.org/obo/GAZ_00021800">
        <rdf:type rdf:resource="http://purl.obolibrary.org/obo/ENVO_00000004"/>
        <obo:RO_0001025 rdf:resource="http://purl.obolibrary.org/obo/GAZ_00010644"/>
        <obo:IAO_0000115>A district in Parvan Province, Afghanistan.</obo:IAO_0000115>
        <oboInOwl:hasOBONamespace>GAZ</oboInOwl:hasOBONamespace>
        <oboInOwl:id>GAZ:00021800</oboInOwl:id>
        <rdfs:label>Salang District</rdfs:label>
    </owl:NamedIndividual>
    


    <!-- http://purl.obolibrary.org/obo/GAZ_00021801 -->

    <owl:NamedIndividual rdf:about="http://purl.obolibrary.org/obo/GAZ_00021801">
        <rdf:type rdf:resource="http://purl.obolibrary.org/obo/ENVO_00000004"/>
        <obo:RO_0001025 rdf:resource="http://purl.obolibrary.org/obo/GAZ_00010645"/>
        <obo:IAO_0000115>A district of Paktika Province, Afghanistan.</obo:IAO_0000115>
        <oboInOwl:hasOBONamespace>GAZ</oboInOwl:hasOBONamespace>
        <oboInOwl:id>GAZ:00021801</oboInOwl:id>
        <rdfs:label>Barmal District</rdfs:label>
    </owl:NamedIndividual>
    


    <!-- http://purl.obolibrary.org/obo/GAZ_00021802 -->

    <owl:NamedIndividual rdf:about="http://purl.obolibrary.org/obo/GAZ_00021802">
        <rdf:type rdf:resource="http://purl.obolibrary.org/obo/ENVO_00000004"/>
        <obo:RO_0001025 rdf:resource="http://purl.obolibrary.org/obo/GAZ_00010645"/>
        <obo:IAO_0000115>A district of Paktika Province, Afghanistan.</obo:IAO_0000115>
        <oboInOwl:hasOBONamespace>GAZ</oboInOwl:hasOBONamespace>
        <oboInOwl:id>GAZ:00021802</oboInOwl:id>
        <rdfs:label>Sarobi District</rdfs:label>
    </owl:NamedIndividual>
    


    <!-- http://purl.obolibrary.org/obo/GAZ_00021803 -->

    <owl:NamedIndividual rdf:about="http://purl.obolibrary.org/obo/GAZ_00021803">
        <rdf:type rdf:resource="http://purl.obolibrary.org/obo/ENVO_00000004"/>
        <obo:RO_0001025 rdf:resource="http://purl.obolibrary.org/obo/GAZ_00010645"/>
        <obo:IAO_0000115>A district of Paktika Province, Afghanistan.</obo:IAO_0000115>
        <oboInOwl:hasOBONamespace>GAZ</oboInOwl:hasOBONamespace>
        <oboInOwl:id>GAZ:00021803</oboInOwl:id>
        <rdfs:label>Waza Khwa District</rdfs:label>
    </owl:NamedIndividual>
    


    <!-- http://purl.obolibrary.org/obo/GAZ_00021804 -->

    <owl:NamedIndividual rdf:about="http://purl.obolibrary.org/obo/GAZ_00021804">
        <rdf:type rdf:resource="http://purl.obolibrary.org/obo/ENVO_00000004"/>
        <obo:RO_0001025 rdf:resource="http://purl.obolibrary.org/obo/GAZ_00010645"/>
        <obo:IAO_0000115>A district of Paktika Province, Afghanistan.</obo:IAO_0000115>
        <oboInOwl:hasOBONamespace>GAZ</oboInOwl:hasOBONamespace>
        <oboInOwl:id>GAZ:00021804</oboInOwl:id>
        <rdfs:label>Sharan District</rdfs:label>
    </owl:NamedIndividual>
    


    <!-- http://purl.obolibrary.org/obo/GAZ_00021805 -->

    <owl:NamedIndividual rdf:about="http://purl.obolibrary.org/obo/GAZ_00021805">
        <rdf:type rdf:resource="http://purl.obolibrary.org/obo/ENVO_00000004"/>
        <obo:RO_0001025 rdf:resource="http://purl.obolibrary.org/obo/GAZ_00010645"/>
        <obo:IAO_0000115>A district of Paktika Province, Afghanistan.</obo:IAO_0000115>
        <oboInOwl:hasOBONamespace>GAZ</oboInOwl:hasOBONamespace>
        <oboInOwl:id>GAZ:00021805</oboInOwl:id>
        <rdfs:label>Gomal District</rdfs:label>
    </owl:NamedIndividual>
    


    <!-- http://purl.obolibrary.org/obo/GAZ_00021806 -->

    <owl:NamedIndividual rdf:about="http://purl.obolibrary.org/obo/GAZ_00021806">
        <rdf:type rdf:resource="http://purl.obolibrary.org/obo/ENVO_00000004"/>
        <obo:RO_0001025 rdf:resource="http://purl.obolibrary.org/obo/GAZ_00010645"/>
        <obo:IAO_0000115>A district of Paktika Province, Afghanistan.</obo:IAO_0000115>
        <oboInOwl:hasOBONamespace>GAZ</oboInOwl:hasOBONamespace>
        <oboInOwl:id>GAZ:00021806</oboInOwl:id>
        <rdfs:label>Urgun District</rdfs:label>
    </owl:NamedIndividual>
    


    <!-- http://purl.obolibrary.org/obo/GAZ_00021807 -->

    <owl:NamedIndividual rdf:about="http://purl.obolibrary.org/obo/GAZ_00021807">
        <rdf:type rdf:resource="http://purl.obolibrary.org/obo/ENVO_00000004"/>
        <obo:RO_0001025 rdf:resource="http://purl.obolibrary.org/obo/GAZ_00010645"/>
        <obo:IAO_0000115>A district of Paktika Province, Afghanistan.</obo:IAO_0000115>
        <oboInOwl:hasOBONamespace>GAZ</oboInOwl:hasOBONamespace>
        <oboInOwl:id>GAZ:00021807</oboInOwl:id>
        <rdfs:label>Mata Khan District</rdfs:label>
    </owl:NamedIndividual>
    


    <!-- http://purl.obolibrary.org/obo/GAZ_00021808 -->

    <owl:NamedIndividual rdf:about="http://purl.obolibrary.org/obo/GAZ_00021808">
        <rdf:type rdf:resource="http://purl.obolibrary.org/obo/ENVO_00000004"/>
        <obo:RO_0001025 rdf:resource="http://purl.obolibrary.org/obo/GAZ_00010645"/>
        <obo:IAO_0000115>A district of Paktika Province, Afghanistan.</obo:IAO_0000115>
        <oboInOwl:hasOBONamespace>GAZ</oboInOwl:hasOBONamespace>
        <oboInOwl:id>GAZ:00021808</oboInOwl:id>
        <rdfs:label>Sar Hawza District</rdfs:label>
    </owl:NamedIndividual>
    


    <!-- http://purl.obolibrary.org/obo/GAZ_00021809 -->

    <owl:NamedIndividual rdf:about="http://purl.obolibrary.org/obo/GAZ_00021809">
        <rdf:type rdf:resource="http://purl.obolibrary.org/obo/ENVO_00000004"/>
        <obo:RO_0001025 rdf:resource="http://purl.obolibrary.org/obo/GAZ_00010645"/>
        <obo:IAO_0000115>A district of Paktika Province, Afghanistan.</obo:IAO_0000115>
        <oboInOwl:hasOBONamespace>GAZ</oboInOwl:hasOBONamespace>
        <oboInOwl:id>GAZ:00021809</oboInOwl:id>
        <rdfs:label>Nika District</rdfs:label>
    </owl:NamedIndividual>
    


    <!-- http://purl.obolibrary.org/obo/GAZ_00021810 -->

    <owl:NamedIndividual rdf:about="http://purl.obolibrary.org/obo/GAZ_00021810">
        <rdf:type rdf:resource="http://purl.obolibrary.org/obo/ENVO_00000004"/>
        <obo:RO_0001025 rdf:resource="http://purl.obolibrary.org/obo/GAZ_00010645"/>
        <obo:IAO_0000115>A district of Paktika Province, Afghanistan.</obo:IAO_0000115>
        <oboInOwl:hasOBONamespace>GAZ</oboInOwl:hasOBONamespace>
        <oboInOwl:id>GAZ:00021810</oboInOwl:id>
        <rdfs:label>Omna District</rdfs:label>
    </owl:NamedIndividual>
    


    <!-- http://purl.obolibrary.org/obo/GAZ_00021811 -->

    <owl:NamedIndividual rdf:about="http://purl.obolibrary.org/obo/GAZ_00021811">
        <rdf:type rdf:resource="http://purl.obolibrary.org/obo/ENVO_00000004"/>
        <obo:RO_0001025 rdf:resource="http://purl.obolibrary.org/obo/GAZ_00010645"/>
        <obo:IAO_0000115>A district of Paktika Province, Afghanistan.</obo:IAO_0000115>
        <oboInOwl:hasOBONamespace>GAZ</oboInOwl:hasOBONamespace>
        <oboInOwl:id>GAZ:00021811</oboInOwl:id>
        <rdfs:label>Dila District</rdfs:label>
    </owl:NamedIndividual>
    


    <!-- http://purl.obolibrary.org/obo/GAZ_00021812 -->

    <owl:NamedIndividual rdf:about="http://purl.obolibrary.org/obo/GAZ_00021812">
        <rdf:type rdf:resource="http://purl.obolibrary.org/obo/ENVO_00000004"/>
        <obo:RO_0001025 rdf:resource="http://purl.obolibrary.org/obo/GAZ_00010645"/>
        <obo:IAO_0000115>A district of Paktika Province, Afghanistan.</obo:IAO_0000115>
        <oboInOwl:hasOBONamespace>GAZ</oboInOwl:hasOBONamespace>
        <oboInOwl:id>GAZ:00021812</oboInOwl:id>
        <rdfs:label>Gayan District</rdfs:label>
    </owl:NamedIndividual>
    


    <!-- http://purl.obolibrary.org/obo/GAZ_00051188 -->

    <owl:NamedIndividual rdf:about="http://purl.obolibrary.org/obo/GAZ_00051188">
        <obo:IAO_0000115>The lowest part of the Sistan Basin; separated from the main basin by a land barrier so it receives runoff water only when the main tributaries are overflowing.</obo:IAO_0000115>
        <oboInOwl:hasOBONamespace>GAZ</oboInOwl:hasOBONamespace>
        <oboInOwl:id>GAZ:00051188</oboInOwl:id>
        <rdfs:label>Godzareh Depression</rdfs:label>
    </owl:NamedIndividual>
    


    <!-- http://purl.obolibrary.org/obo/GAZ_00053737 -->

    <owl:NamedIndividual rdf:about="http://purl.obolibrary.org/obo/GAZ_00053737">
        <rdf:type rdf:resource="http://purl.obolibrary.org/obo/ENVO_00000354"/>
        <obo:RO_0001025 rdf:resource="http://purl.obolibrary.org/obo/GAZ_00006882"/>
        <obo:IAO_0000115>A volcanic group that consists of 18 dacitic and trachytic volcanoes located WSW of Kabul. It is the northernmost of a group of small volcanic fields in the Ghanzi region and consists of endogenous lava domes, one of which occupies an old caldera.</obo:IAO_0000115>
        <oboInOwl:hasOBONamespace>GAZ</oboInOwl:hasOBONamespace>
        <oboInOwl:id>GAZ:00053737</oboInOwl:id>
        <rdfs:label>Vakak Volcanic Field</rdfs:label>
    </owl:NamedIndividual>
    


    <!-- http://purl.obolibrary.org/obo/GAZ_00053738 -->

    <owl:NamedIndividual rdf:about="http://purl.obolibrary.org/obo/GAZ_00053738">
        <obo:RO_0001025 rdf:resource="http://purl.obolibrary.org/obo/GAZ_00006882"/>
        <obo:IAO_0000115>A volcanic field that is a group of 15 trachyandesitic lava domes located in west-central Afghanistan SW of Kabul. The domes lie along the southern margin of Dacht-i-Navar.</obo:IAO_0000115>
        <oboInOwl:hasOBONamespace>GAZ</oboInOwl:hasOBONamespace>
        <oboInOwl:id>GAZ:00053738</oboInOwl:id>
        <rdfs:label>Dacht-i-Navar Volcanic Field</rdfs:label>
    </owl:NamedIndividual>
    


    <!-- http://purl.obolibrary.org/obo/GAZ_00056902 -->

    <owl:NamedIndividual rdf:about="http://purl.obolibrary.org/obo/GAZ_00056902">
        <obo:IAO_0000115>A mountain range in Afghanistan as well as in the North-West Frontier Province and Northern Areas of Pakistan. It is the westernmost extension of the Pamir Mountains, the Karakoram Range, and the Himalayas.</obo:IAO_0000115>
        <oboInOwl:hasOBONamespace>GAZ</oboInOwl:hasOBONamespace>
        <oboInOwl:id>GAZ:00056902</oboInOwl:id>
        <rdfs:label>Hindu Kush</rdfs:label>
    </owl:NamedIndividual>
    


    <!-- http://purl.obolibrary.org/obo/GAZ_00056903 -->

    <owl:NamedIndividual rdf:about="http://purl.obolibrary.org/obo/GAZ_00056903">
        <rdf:type rdf:resource="http://purl.obolibrary.org/obo/ENVO_00000104"/>
        <rdf:type rdf:resource="http://purl.obolibrary.org/obo/ENVO_00000106"/>
        <obo:RO_0001025 rdf:resource="http://purl.obolibrary.org/obo/GAZ_00006882"/>
        <obo:IAO_0000115>A range of mountains on the Pakistan-Afghanistan border, up to 15,620ft (4,761 m) above sea-level at Mount Sikaram, straight and rigid, towering above all surrounding hills, it is near the Kabul River. A spur of the range is crossed by the Khyber Pass.</obo:IAO_0000115>
        <oboInOwl:hasOBONamespace>GAZ</oboInOwl:hasOBONamespace>
        <oboInOwl:id>GAZ:00056903</oboInOwl:id>
        <rdfs:label>Safed Koh Mountains</rdfs:label>
    </owl:NamedIndividual>
    


    <!-- http://purl.obolibrary.org/obo/GAZ_00057344 -->

    <owl:NamedIndividual rdf:about="http://purl.obolibrary.org/obo/GAZ_00057344">
        <obo:IAO_0000115>A subrange of the Himalayas spanning part of the border between Tibet and Nepal. It contains four eight-thousanders: Mount Everest, Lhotse, Makalu, and Cho Oyu, as well as numerous other major peaks.</obo:IAO_0000115>
        <oboInOwl:hasOBONamespace>GAZ</oboInOwl:hasOBONamespace>
        <oboInOwl:id>GAZ:00057344</oboInOwl:id>
        <rdfs:label>Mahalangur Himal</rdfs:label>
    </owl:NamedIndividual>
    


    <!-- http://purl.obolibrary.org/obo/GAZ_00057359 -->

    <owl:NamedIndividual rdf:about="http://purl.obolibrary.org/obo/GAZ_00057359">
        <obo:IAO_0000115>A mountain range that is a southern branch of the main Himalayan chain of mountains. It rises spectacularly from the Indian plains to the north of Kangra and Mandi.</obo:IAO_0000115>
        <oboInOwl:hasOBONamespace>GAZ</oboInOwl:hasOBONamespace>
        <oboInOwl:id>GAZ:00057359</oboInOwl:id>
        <rdfs:label>Dhauladhar Range</rdfs:label>
    </owl:NamedIndividual>
    


    <!-- http://purl.obolibrary.org/obo/GAZ_00057373 -->

    <owl:NamedIndividual rdf:about="http://purl.obolibrary.org/obo/GAZ_00057373">
        <rdf:type rdf:resource="http://purl.obolibrary.org/obo/ENVO_00000106"/>
        <obo:IAO_0000115>A range of mountains that form a part of the Middle Himalayas across the two states of Jammu and Kashmir and Himachal Pradesh in India as well as Azad Kashmir, Pakistan.</obo:IAO_0000115>
        <oboInOwl:hasOBONamespace>GAZ</oboInOwl:hasOBONamespace>
        <oboInOwl:id>GAZ:00057373</oboInOwl:id>
        <rdfs:label>Pir Panjal Range</rdfs:label>
    </owl:NamedIndividual>
    


    <!-- http://purl.obolibrary.org/obo/GAZ_00057374 -->

    <owl:NamedIndividual rdf:about="http://purl.obolibrary.org/obo/GAZ_00057374">
        <obo:IAO_0000115>A mountain range that lies north of the Sub-Himalayan Range and south of the Great Himalayas. In Pakistan these mountains lie just north of Rawalpindi district covering the districts of Batagram, Mansehra and Abbottabad as well as Pakistan Administered Kashmir. These mountains are also home to Pakistan&apos;s important hill stations like Murree, Ghora Gali and Nathia Gali. It snows here during a few months of the year but there aren&apos;t any glaciers found in this region. The range continues east through the Indian states of Jammu and Kashmir, Himachal Pradesh, Uttarakhand, Uttar Pradesh. The range then enters the countries of Nepal and Bhutan, and then enters the eastern Indian states of West Bengal, Sikkim, Assam and Arunachal Pradesh.</obo:IAO_0000115>
        <oboInOwl:hasOBONamespace>GAZ</oboInOwl:hasOBONamespace>
        <oboInOwl:id>GAZ:00057374</oboInOwl:id>
        <rdfs:label>Lower Himalayan Range</rdfs:label>
    </owl:NamedIndividual>
    


    <!-- http://purl.obolibrary.org/obo/GAZ_00057375 -->

    <owl:NamedIndividual rdf:about="http://purl.obolibrary.org/obo/GAZ_00057375">
        <obo:IAO_0000115>The southernmost mountains in the Himalaya Range. Their average height varies between 600 to 1200 meters, and are not so high in altitude as compared to other mountain ranges in the Himalaya range. These mountains are well spread in Kashmir, in Pakistan however they are located south-east of the Rawalpindi district.</obo:IAO_0000115>
        <oboInOwl:hasOBONamespace>GAZ</oboInOwl:hasOBONamespace>
        <oboInOwl:id>GAZ:00057375</oboInOwl:id>
        <rdfs:label>Sub-Himalayan Range</rdfs:label>
    </owl:NamedIndividual>
    


    <!-- http://purl.obolibrary.org/obo/GAZ_00057376 -->

    <owl:NamedIndividual rdf:about="http://purl.obolibrary.org/obo/GAZ_00057376">
        <obo:IAO_0000115>A mountain range that lies north of the Lower Himalayan Range. These mountains are bounded by the Indus River in the north and the west as the river takes a southward turn at Sazin. The average height of the range is about 6000 meters. Some of the highest peaks in the world lie in these mountains e.g. Nanga Parbat (8126 meters), which is the sixth highest peak in the world and the second highest peak in Pakistan. Since the mountains are perpetually covered with snow there are many glaciers, with Rupal Glacier being the longest (17.6 km).</obo:IAO_0000115>
        <oboInOwl:hasOBONamespace>GAZ</oboInOwl:hasOBONamespace>
        <oboInOwl:id>GAZ:00057376</oboInOwl:id>
        <rdfs:label>Great Himalayas</rdfs:label>
    </owl:NamedIndividual>
    


    <!-- http://purl.obolibrary.org/obo/GAZ_00057421 -->

    <owl:NamedIndividual rdf:about="http://purl.obolibrary.org/obo/GAZ_00057421">
        <obo:IAO_0000115>A mountains in the north of Thailand that extend through Laos, Burma and China to link to the Himalayas, of which they may be considered foothills.</obo:IAO_0000115>
        <oboInOwl:hasOBONamespace>GAZ</oboInOwl:hasOBONamespace>
        <oboInOwl:id>GAZ:00057421</oboInOwl:id>
        <rdfs:label>Thai Highlands</rdfs:label>
    </owl:NamedIndividual>
    


    <!-- http://purl.obolibrary.org/obo/GAZ_00057450 -->

    <owl:NamedIndividual rdf:about="http://purl.obolibrary.org/obo/GAZ_00057450">
        <obo:RO_0001025 rdf:resource="http://purl.obolibrary.org/obo/GAZ_00004988"/>
        <obo:IAO_0000115>A mountain range in the Western Pamirs of Tajikistan. The length of the Akademiya Nauk Range is about 110 km. The crest of the range has an Alpine-like relief with 24 summits more than 6,000 m in height. The lowest saddle point, Kamaloyak is at the altitude of 4,340 m.</obo:IAO_0000115>
        <oboInOwl:hasOBONamespace>GAZ</oboInOwl:hasOBONamespace>
        <oboInOwl:id>GAZ:00057450</oboInOwl:id>
        <rdfs:label>Akademiya Nauk Range</rdfs:label>
    </owl:NamedIndividual>
    


    <!-- http://purl.obolibrary.org/obo/GAZ_00057453 -->

    <owl:NamedIndividual rdf:about="http://purl.obolibrary.org/obo/GAZ_00057453">
        <obo:IAO_0000115>A traditional designation for the portion of the Himalaya range between the eastern border of Bhutan, on the west, and the Great Bend of the Tsangpo River, on the east.</obo:IAO_0000115>
        <oboInOwl:hasOBONamespace>GAZ</oboInOwl:hasOBONamespace>
        <oboInOwl:id>GAZ:00057453</oboInOwl:id>
        <rdfs:label>Assam Himalaya</rdfs:label>
    </owl:NamedIndividual>
    


    <!-- http://purl.obolibrary.org/obo/GAZ_00057455 -->

    <owl:NamedIndividual rdf:about="http://purl.obolibrary.org/obo/GAZ_00057455">
        <obo:IAO_0000115>A sub-range of the Himalayan mountain range. It is located mostly in north-central Nepal, but some peaks lie on the border with Tibet. The Trisuli Gandaki valley on the east separates it from the Langtang Himal; the Budhi Gandaki valley and the Shyar Khola valley on the west separate it from the Sringi Himal and the Mansiri Himal (home of Manaslu, the nearest 8000m peak). The range lies about 70 km north-northwest of Kathmandu.</obo:IAO_0000115>
        <oboInOwl:hasOBONamespace>GAZ</oboInOwl:hasOBONamespace>
        <oboInOwl:id>GAZ:00057455</oboInOwl:id>
        <rdfs:label>Ganesh Himal</rdfs:label>
    </owl:NamedIndividual>
    


    <!-- http://purl.obolibrary.org/obo/GAZ_00057456 -->

    <owl:NamedIndividual rdf:about="http://purl.obolibrary.org/obo/GAZ_00057456">
        <oboInOwl:hasOBONamespace>GAZ</oboInOwl:hasOBONamespace>
        <oboInOwl:id>GAZ:00057456</oboInOwl:id>
        <rdfs:label>Langtang Himal</rdfs:label>
    </owl:NamedIndividual>
    


    <!-- http://purl.obolibrary.org/obo/GAZ_00057457 -->

    <owl:NamedIndividual rdf:about="http://purl.obolibrary.org/obo/GAZ_00057457">
        <oboInOwl:hasOBONamespace>GAZ</oboInOwl:hasOBONamespace>
        <oboInOwl:id>GAZ:00057457</oboInOwl:id>
        <rdfs:label>Sringi Himal</rdfs:label>
    </owl:NamedIndividual>
    


    <!-- http://purl.obolibrary.org/obo/GAZ_00057459 -->

    <owl:NamedIndividual rdf:about="http://purl.obolibrary.org/obo/GAZ_00057459">
        <obo:IAO_0000115>A small, high subrange of the Himalaya in north-central Nepal. It rises between the Marsyangdi River on the west, and the Burhi (Budhi) Gandaki on the east, and lies roughly 100 km northwest of Kathmandu. To the west lies the Annapurna Himal, and to the east is the Ganesh Himal.</obo:IAO_0000115>
        <oboInOwl:hasOBONamespace>GAZ</oboInOwl:hasOBONamespace>
        <oboInOwl:id>GAZ:00057459</oboInOwl:id>
        <rdfs:label>Mansiri Himal</rdfs:label>
    </owl:NamedIndividual>
    


    <!-- http://purl.obolibrary.org/obo/GAZ_00057460 -->

    <owl:NamedIndividual rdf:about="http://purl.obolibrary.org/obo/GAZ_00057460">
        <obo:IAO_0000115>A series of peaks in the Himalaya, a 55 km ong massif whose highest point, Annapurna I, stands at 8,091 m making it the 10th-highest summit in the world. It is located east of a great gorge cut through the Himalaya by the Kali Gandaki River, which separates it from the Dhaulagiri massif.</obo:IAO_0000115>
        <oboInOwl:hasOBONamespace>GAZ</oboInOwl:hasOBONamespace>
        <oboInOwl:id>GAZ:00057460</oboInOwl:id>
        <rdfs:label>Annapurna Himal</rdfs:label>
    </owl:NamedIndividual>
    


    <!-- http://purl.obolibrary.org/obo/GAZ_00057461 -->

    <owl:NamedIndividual rdf:about="http://purl.obolibrary.org/obo/GAZ_00057461">
        <obo:IAO_0000115>A small subrange of the Himalayan range in southern Tibet and the northwest corner of Nepal. It lies south of Lake Manasarowar. Its southern boundary is the Humla Karnali, a tributary of the Karnali, one of the major rivers of western Nepal. This river separates the range from the Gurans Himal to the south and the eastern Kumaon to the southwest. On the east, the pass known as Lapche La marks the dividing point between the Nalakankar Himal and the Chandi Himal. To the north and northwest, the range fades into the northern foothills of the Himalaya and the Tibetan Plateau.</obo:IAO_0000115>
        <oboInOwl:hasOBONamespace>GAZ</oboInOwl:hasOBONamespace>
        <oboInOwl:id>GAZ:00057461</oboInOwl:id>
        <rdfs:label>Nalakankar Himal</rdfs:label>
    </owl:NamedIndividual>
    


    <!-- http://purl.obolibrary.org/obo/GAZ_00057462 -->

    <owl:NamedIndividual rdf:about="http://purl.obolibrary.org/obo/GAZ_00057462">
        <obo:IAO_0000115>A sub-range of the Himalaya, located in north central Nepal and extending into south central Tibet. The range is bounded on the south by the Rolwaling Valley.</obo:IAO_0000115>
        <oboInOwl:hasOBONamespace>GAZ</oboInOwl:hasOBONamespace>
        <oboInOwl:id>GAZ:00057462</oboInOwl:id>
        <rdfs:label>Rolwaling Himal</rdfs:label>
    </owl:NamedIndividual>
    


    <!-- http://purl.obolibrary.org/obo/GAZ_00057463 -->

    <owl:NamedIndividual rdf:about="http://purl.obolibrary.org/obo/GAZ_00057463">
        <obo:IAO_0000115>A small subrange of the Himalaya in far western Nepal.</obo:IAO_0000115>
        <oboInOwl:hasOBONamespace>GAZ</oboInOwl:hasOBONamespace>
        <oboInOwl:id>GAZ:00057463</oboInOwl:id>
        <rdfs:label>Gurans Himal</rdfs:label>
    </owl:NamedIndividual>
    


    <!-- http://purl.obolibrary.org/obo/GAZ_00057464 -->

    <owl:NamedIndividual rdf:about="http://purl.obolibrary.org/obo/GAZ_00057464">
        <obo:IAO_0000115>A subrange of the Himalaya in the Dhawalagiri Zone of north central Nepal.</obo:IAO_0000115>
        <oboInOwl:hasOBONamespace>GAZ</oboInOwl:hasOBONamespace>
        <oboInOwl:id>GAZ:00057464</oboInOwl:id>
        <rdfs:label>Dhaulagiri Himal</rdfs:label>
    </owl:NamedIndividual>
    


    <!-- http://purl.obolibrary.org/obo/GAZ_00057491 -->

    <owl:NamedIndividual rdf:about="http://purl.obolibrary.org/obo/GAZ_00057491">
        <obo:RO_0001025 rdf:resource="http://purl.obolibrary.org/obo/GAZ_00004988"/>
        <obo:IAO_0000115>A mountain range of the Pamir Mountains (ancient Mount Imeon) between Kyrgyzstan and Tajikistan. Its northern end is the Alay Valley, and 150 miles to the south, it terminates into the valleys of Muksu and Markansu. The highest peak in the range is Lenin Peak.</obo:IAO_0000115>
        <oboInOwl:hasOBONamespace>GAZ</oboInOwl:hasOBONamespace>
        <oboInOwl:id>GAZ:00057491</oboInOwl:id>
        <rdfs:label>Trans-Alay Range</rdfs:label>
    </owl:NamedIndividual>
    


    <!-- http://purl.obolibrary.org/obo/GAZ_00057740 -->

    <owl:NamedIndividual rdf:about="http://purl.obolibrary.org/obo/GAZ_00057740">
        <obo:RO_0001025 rdf:resource="http://purl.obolibrary.org/obo/GAZ_00010642"/>
        <obo:RO_0001025 rdf:resource="http://purl.obolibrary.org/obo/GAZ_00010650"/>
        <obo:IAO_0000115>An extremely arid plateau region located between Helmand and Kandahar provinces in southwestern Afghanistan.</obo:IAO_0000115>
        <oboInOwl:hasOBONamespace>GAZ</oboInOwl:hasOBONamespace>
        <oboInOwl:id>GAZ:00057740</oboInOwl:id>
        <rdfs:label>Registan Desert</rdfs:label>
    </owl:NamedIndividual>
    


    <!-- http://purl.obolibrary.org/obo/GAZ_00058024 -->

    <owl:NamedIndividual rdf:about="http://purl.obolibrary.org/obo/GAZ_00058024">
        <obo:RO_0001025 rdf:resource="http://purl.obolibrary.org/obo/GAZ_00010626"/>
        <obo:IAO_0000115>A marshy lake located in southeast Iran near the Afghan border and fed by the Helmand River. Together with Iran&apos;s Hamun-e Puzak and Hamun-e Saber rivers, it forms the extended wetlands of Seistan on the large border region in southeastern Iran and soutwestern Afghanistan. Seasonal tributaries are Halil River and Bampur River.</obo:IAO_0000115>
        <oboInOwl:hasOBONamespace>GAZ</oboInOwl:hasOBONamespace>
        <oboInOwl:id>GAZ:00058024</oboInOwl:id>
        <rdfs:label>Hamun-e Helmand</rdfs:label>
    </owl:NamedIndividual>
    


    <!-- http://purl.obolibrary.org/obo/GAZ_00058025 -->

    <owl:NamedIndividual rdf:about="http://purl.obolibrary.org/obo/GAZ_00058025">
        <obo:RO_0001025 rdf:resource="http://purl.obolibrary.org/obo/GAZ_00056902"/>
        <obo:RO_0001025 rdf:resource="http://purl.obolibrary.org/obo/GAZ_00076852"/>
        <obo:IAO_0000115>A group of lakes high in the Hindu Kush Mountains of Central Afghanistan near the famous Buddhas of Bamyan. They were created by the carbon dioxide rich water oozing out of the faults and fractures to deposit calcium carbonate precipitate in the form of travertine walls that today store the water of these lakes. Band-e Amir is situated at approximately 75 km to the north-west of the ancient city of Bamyan, close the town of Yakawlang.</obo:IAO_0000115>
        <oboInOwl:hasOBONamespace>GAZ</oboInOwl:hasOBONamespace>
        <oboInOwl:id>GAZ:00058025</oboInOwl:id>
        <rdfs:label>Band-e Amir</rdfs:label>
    </owl:NamedIndividual>
    


    <!-- http://purl.obolibrary.org/obo/GAZ_00058026 -->

    <owl:NamedIndividual rdf:about="http://purl.obolibrary.org/obo/GAZ_00058026">
        <obo:RO_0001025 rdf:resource="http://purl.obolibrary.org/obo/GAZ_00058025"/>
        <obo:IAO_0000115>One of the Band-e Amir lakes.</obo:IAO_0000115>
        <oboInOwl:hasOBONamespace>GAZ</oboInOwl:hasOBONamespace>
        <oboInOwl:id>GAZ:00058026</oboInOwl:id>
        <rdfs:label>Band-e Haibat</rdfs:label>
    </owl:NamedIndividual>
    


    <!-- http://purl.obolibrary.org/obo/GAZ_00058027 -->

    <owl:NamedIndividual rdf:about="http://purl.obolibrary.org/obo/GAZ_00058027">
        <obo:RO_0001025 rdf:resource="http://purl.obolibrary.org/obo/GAZ_00058025"/>
        <obo:IAO_0000115>One of the Band-e Amir lakes.</obo:IAO_0000115>
        <oboInOwl:hasOBONamespace>GAZ</oboInOwl:hasOBONamespace>
        <oboInOwl:id>GAZ:00058027</oboInOwl:id>
        <rdfs:label>Band-e Qambar</rdfs:label>
    </owl:NamedIndividual>
    


    <!-- http://purl.obolibrary.org/obo/GAZ_00058028 -->

    <owl:NamedIndividual rdf:about="http://purl.obolibrary.org/obo/GAZ_00058028">
        <obo:RO_0001025 rdf:resource="http://purl.obolibrary.org/obo/GAZ_00058025"/>
        <obo:IAO_0000115>One of the Band-e Amir lakes.</obo:IAO_0000115>
        <oboInOwl:hasOBONamespace>GAZ</oboInOwl:hasOBONamespace>
        <oboInOwl:id>GAZ:00058028</oboInOwl:id>
        <rdfs:label>Band-e Zulfiqar</rdfs:label>
    </owl:NamedIndividual>
    


    <!-- http://purl.obolibrary.org/obo/GAZ_00058029 -->

    <owl:NamedIndividual rdf:about="http://purl.obolibrary.org/obo/GAZ_00058029">
        <obo:RO_0001025 rdf:resource="http://purl.obolibrary.org/obo/GAZ_00058025"/>
        <obo:IAO_0000115>One of the Band-e Amir lakes.</obo:IAO_0000115>
        <oboInOwl:hasOBONamespace>GAZ</oboInOwl:hasOBONamespace>
        <oboInOwl:id>GAZ:00058029</oboInOwl:id>
        <rdfs:label>Band-e Pudina</rdfs:label>
    </owl:NamedIndividual>
    


    <!-- http://purl.obolibrary.org/obo/GAZ_00058030 -->

    <owl:NamedIndividual rdf:about="http://purl.obolibrary.org/obo/GAZ_00058030">
        <obo:RO_0001025 rdf:resource="http://purl.obolibrary.org/obo/GAZ_00058025"/>
        <obo:IAO_0000115>One of the Band-e Amir lakes.</obo:IAO_0000115>
        <oboInOwl:hasOBONamespace>GAZ</oboInOwl:hasOBONamespace>
        <oboInOwl:id>GAZ:00058030</oboInOwl:id>
        <rdfs:label>Band-e Panir</rdfs:label>
    </owl:NamedIndividual>
    


    <!-- http://purl.obolibrary.org/obo/GAZ_00058031 -->

    <owl:NamedIndividual rdf:about="http://purl.obolibrary.org/obo/GAZ_00058031">
        <obo:RO_0001025 rdf:resource="http://purl.obolibrary.org/obo/GAZ_00058025"/>
        <obo:IAO_0000115>One of the Band-e Amir lakes.</obo:IAO_0000115>
        <oboInOwl:hasOBONamespace>GAZ</oboInOwl:hasOBONamespace>
        <oboInOwl:id>GAZ:00058031</oboInOwl:id>
        <rdfs:label>Band-e Gholaman</rdfs:label>
    </owl:NamedIndividual>
    


    <!-- http://purl.obolibrary.org/obo/GAZ_00058032 -->

    <owl:NamedIndividual rdf:about="http://purl.obolibrary.org/obo/GAZ_00058032">
        <obo:RO_0001025 rdf:resource="http://purl.obolibrary.org/obo/GAZ_00004988"/>
        <obo:RO_0001025 rdf:resource="http://purl.obolibrary.org/obo/GAZ_00098853"/>
        <obo:IAO_0000115>A lake in the Pamir Mountains. It extends east to west for about 25 km. Along the western half of the lake runs the Afghan-Tajik border, turning south towards Concord Peak (5,469 m), about 15 km south of the lake. The lake&apos;s eastern half lies in Tajikistan. Out of the lake, towards the west, flows Pamir River.</obo:IAO_0000115>
        <oboInOwl:hasOBONamespace>GAZ</oboInOwl:hasOBONamespace>
        <oboInOwl:id>GAZ:00058032</oboInOwl:id>
        <rdfs:label>Zorkul</rdfs:label>
    </owl:NamedIndividual>
    


    <!-- http://purl.obolibrary.org/obo/GAZ_00058368 -->

    <owl:NamedIndividual rdf:about="http://purl.obolibrary.org/obo/GAZ_00058368">
        <obo:IAO_0000115>The southernmost and geologically youngest east-west mountain chain of the Himalayan System. The Sivalik Hills crest at 900 to 1,200 meters and have many sub-ranges. They extend 1,600 km from the Teesta River in Sikkim, westward through Nepal and Uttarakhand, continuing into Kashmir and Northern Pakistan. The Mohan Pass is the principal pass accessing the Sivalik Hills from Saharanpur in Uttar Pradesh to Dehra and the hill station of Mussoorie in Uttarakhand. Eastward they are cut through at wide intervals by large rivers flowing south from the Himalaya.</obo:IAO_0000115>
        <oboInOwl:hasOBONamespace>GAZ</oboInOwl:hasOBONamespace>
        <oboInOwl:id>GAZ:00058368</oboInOwl:id>
        <rdfs:label>Sivalik Hills</rdfs:label>
    </owl:NamedIndividual>
    


    <!-- http://purl.obolibrary.org/obo/GAZ_00058373 -->

    <owl:NamedIndividual rdf:about="http://purl.obolibrary.org/obo/GAZ_00058373">
        <obo:RO_0001025 rdf:resource="http://purl.obolibrary.org/obo/GAZ_00057460"/>
        <obo:IAO_0000115>One of the highest lakes in the world in the Annapurna Himal. A tarn, a lake caused by glacial activity.</obo:IAO_0000115>
        <oboInOwl:hasOBONamespace>GAZ</oboInOwl:hasOBONamespace>
        <oboInOwl:id>GAZ:00058373</oboInOwl:id>
        <rdfs:label>Tilicho Lake</rdfs:label>
    </owl:NamedIndividual>
    


    <!-- http://purl.obolibrary.org/obo/GAZ_00058498 -->

    <owl:NamedIndividual rdf:about="http://purl.obolibrary.org/obo/GAZ_00058498">
        <obo:RO_0001025 rdf:resource="http://purl.obolibrary.org/obo/GAZ_00004988"/>
        <obo:IAO_0000115>A 25 km diameter crater lake in the Pamir Mountains in Tajikistan, which lies at an altitude of 3,900 meters (13,000 feet) above mean sea level. A peninsula projecting from the south shore and an island off the north shore divide the lake into two basins, a smaller eastern one which is relatively shallow, between 13 to 19 meters, and a larger western one, with depths of 221 to 230 meters. It has no drainage outlet. Kara-Kul lake lies within a circular depression interpreted as a meteorite impact crater with a rim diameter of 45 km.</obo:IAO_0000115>
        <oboInOwl:hasOBONamespace>GAZ</oboInOwl:hasOBONamespace>
        <oboInOwl:id>GAZ:00058498</oboInOwl:id>
        <rdfs:label>Kara-Kul</rdfs:label>
    </owl:NamedIndividual>
    


    <!-- http://purl.obolibrary.org/obo/GAZ_00058499 -->

    <owl:NamedIndividual rdf:about="http://purl.obolibrary.org/obo/GAZ_00058499">
        <obo:RO_0001025 rdf:resource="http://purl.obolibrary.org/obo/GAZ_00004988"/>
        <obo:IAO_0000115>A lake in Tajikistan, in the northeast Pamir Mountains, northwest of the Muztagh Ata peak (7,880 metres), at an altitude of 3,870 m. It is a moraine lake; and a stream of the same name flows through it.</obo:IAO_0000115>
        <oboInOwl:hasOBONamespace>GAZ</oboInOwl:hasOBONamespace>
        <oboInOwl:id>GAZ:00058499</oboInOwl:id>
        <rdfs:label>Little Kara-Kul</rdfs:label>
    </owl:NamedIndividual>
    


    <!-- http://purl.obolibrary.org/obo/GAZ_00058500 -->

    <owl:NamedIndividual rdf:about="http://purl.obolibrary.org/obo/GAZ_00058500">
        <obo:IAO_0000115>A Central Asian river, and one of the main rivers of the nation of Tajikistan. It is a tributary of the Amu Darya river. The river&apos;s source lies in Kyrgyzstan; it then flows through Tajikistan for a length of 524 km before joining the Panj River to form the Amu Darya at the border of Tajikistan and Afghanistan.</obo:IAO_0000115>
        <oboInOwl:hasOBONamespace>GAZ</oboInOwl:hasOBONamespace>
        <oboInOwl:id>GAZ:00058500</oboInOwl:id>
        <rdfs:label>Vakhsh River</rdfs:label>
    </owl:NamedIndividual>
    


    <!-- http://purl.obolibrary.org/obo/GAZ_00058501 -->

    <owl:NamedIndividual rdf:about="http://purl.obolibrary.org/obo/GAZ_00058501">
        <obo:RO_0001025 rdf:resource="http://purl.obolibrary.org/obo/GAZ_00058500"/>
        <obo:IAO_0000115>A reservoir formed bu the Nurek Dam on the Vakhsh River in Tajikistan.</obo:IAO_0000115>
        <oboInOwl:hasOBONamespace>GAZ</oboInOwl:hasOBONamespace>
        <oboInOwl:id>GAZ:00058501</oboInOwl:id>
        <rdfs:label>Nurek</rdfs:label>
    </owl:NamedIndividual>
    


    <!-- http://purl.obolibrary.org/obo/GAZ_00058502 -->

    <owl:NamedIndividual rdf:about="http://purl.obolibrary.org/obo/GAZ_00058502">
        <obo:RO_0001025 rdf:resource="http://purl.obolibrary.org/obo/GAZ_00004988"/>
        <obo:IAO_0000115>A lake in Pamir, Tajikistan. The lake formed in 1911, after a great earthquake, when the Murghab River was blocked by a big landslide, forming the Usoi Dam.</obo:IAO_0000115>
        <oboInOwl:hasOBONamespace>GAZ</oboInOwl:hasOBONamespace>
        <oboInOwl:id>GAZ:00058502</oboInOwl:id>
        <rdfs:label>Sarez Lake</rdfs:label>
    </owl:NamedIndividual>
    


    <!-- http://purl.obolibrary.org/obo/GAZ_00058503 -->

    <owl:NamedIndividual rdf:about="http://purl.obolibrary.org/obo/GAZ_00058503">
        <obo:RO_0001025 rdf:resource="http://purl.obolibrary.org/obo/GAZ_00004988"/>
        <obo:IAO_0000115>A natural landslide dam along the Murghab River in the Central Asian nation of Tajikistan. Established 1911-02-18, when a great earthquake estimated between 8 and 9 on the Richter Scale caused a massive landslide to block the flow of the river.</obo:IAO_0000115>
        <oboInOwl:hasOBONamespace>GAZ</oboInOwl:hasOBONamespace>
        <oboInOwl:id>GAZ:00058503</oboInOwl:id>
        <rdfs:label>Usoi Dam</rdfs:label>
    </owl:NamedIndividual>
    


    <!-- http://purl.obolibrary.org/obo/GAZ_00076850 -->

    <owl:NamedIndividual rdf:about="http://purl.obolibrary.org/obo/GAZ_00076850">
        <obo:RO_0001025 rdf:resource="http://purl.obolibrary.org/obo/GAZ_00006882"/>
        <obo:IAO_0000115>A national park in Afghanistan.</obo:IAO_0000115>
        <oboInOwl:hasOBONamespace>GAZ</oboInOwl:hasOBONamespace>
        <oboInOwl:id>GAZ:00076850</oboInOwl:id>
        <rdfs:label>Ab-i-Estada National Park</rdfs:label>
    </owl:NamedIndividual>
    


    <!-- http://purl.obolibrary.org/obo/GAZ_00076851 -->

    <owl:NamedIndividual rdf:about="http://purl.obolibrary.org/obo/GAZ_00076851">
        <obo:RO_0001025 rdf:resource="http://purl.obolibrary.org/obo/GAZ_00006882"/>
        <obo:IAO_0000115>A national park in Afghanistan.</obo:IAO_0000115>
        <oboInOwl:hasOBONamespace>GAZ</oboInOwl:hasOBONamespace>
        <oboInOwl:id>GAZ:00076851</oboInOwl:id>
        <rdfs:label>Ajar Valley National Park</rdfs:label>
    </owl:NamedIndividual>
    


    <!-- http://purl.obolibrary.org/obo/GAZ_00076852 -->

    <owl:NamedIndividual rdf:about="http://purl.obolibrary.org/obo/GAZ_00076852">
        <obo:RO_0001025 rdf:resource="http://purl.obolibrary.org/obo/GAZ_00010657"/>
        <obo:IAO_0000115>A national park in Afghanistan. It lies in the Hazarajat mountains of the western Hindu Kush, Bamiyan Province, some 60 km west of Bamiyan Town.</obo:IAO_0000115>
        <oboInOwl:hasOBONamespace>GAZ</oboInOwl:hasOBONamespace>
        <oboInOwl:id>GAZ:00076852</oboInOwl:id>
        <rdfs:label>Band-e Amir National Park</rdfs:label>
    </owl:NamedIndividual>
    


    <!-- http://purl.obolibrary.org/obo/GAZ_00076853 -->

    <owl:NamedIndividual rdf:about="http://purl.obolibrary.org/obo/GAZ_00076853">
        <obo:RO_0001025 rdf:resource="http://purl.obolibrary.org/obo/GAZ_00006882"/>
        <obo:IAO_0000115>A national park in Afghanistan.</obo:IAO_0000115>
        <oboInOwl:hasOBONamespace>GAZ</oboInOwl:hasOBONamespace>
        <oboInOwl:id>GAZ:00076853</oboInOwl:id>
        <rdfs:label>Nuristan National Park</rdfs:label>
    </owl:NamedIndividual>
    


    <!-- http://purl.obolibrary.org/obo/GAZ_00076854 -->

    <owl:NamedIndividual rdf:about="http://purl.obolibrary.org/obo/GAZ_00076854">
        <obo:RO_0001025 rdf:resource="http://purl.obolibrary.org/obo/GAZ_00006882"/>
        <obo:IAO_0000115>A protected area in Afghanistan.</obo:IAO_0000115>
        <oboInOwl:hasOBONamespace>GAZ</oboInOwl:hasOBONamespace>
        <oboInOwl:id>GAZ:00076854</oboInOwl:id>
        <rdfs:label>Zadran National Reserve</rdfs:label>
    </owl:NamedIndividual>
    


    <!-- http://purl.obolibrary.org/obo/GAZ_00076855 -->

    <owl:NamedIndividual rdf:about="http://purl.obolibrary.org/obo/GAZ_00076855">
        <obo:RO_0001025 rdf:resource="http://purl.obolibrary.org/obo/GAZ_00006882"/>
        <obo:IAO_0000115>A protected area in Afghanistan.</obo:IAO_0000115>
        <oboInOwl:hasOBONamespace>GAZ</oboInOwl:hasOBONamespace>
        <oboInOwl:id>GAZ:00076855</oboInOwl:id>
        <rdfs:label>Darqad (Takhar) Wildlife Managed Reserve</rdfs:label>
    </owl:NamedIndividual>
    


    <!-- http://purl.obolibrary.org/obo/GAZ_00076856 -->

    <owl:NamedIndividual rdf:about="http://purl.obolibrary.org/obo/GAZ_00076856">
        <obo:RO_0001025 rdf:resource="http://purl.obolibrary.org/obo/GAZ_00006882"/>
        <obo:IAO_0000115>A protected area in Afghanistan.</obo:IAO_0000115>
        <oboInOwl:hasOBONamespace>GAZ</oboInOwl:hasOBONamespace>
        <oboInOwl:id>GAZ:00076856</oboInOwl:id>
        <rdfs:label>Imam Sahib (Kunduz) Wildlife Managed Reserve</rdfs:label>
    </owl:NamedIndividual>
    


    <!-- http://purl.obolibrary.org/obo/GAZ_00076857 -->

    <owl:NamedIndividual rdf:about="http://purl.obolibrary.org/obo/GAZ_00076857">
        <obo:RO_0001025 rdf:resource="http://purl.obolibrary.org/obo/GAZ_00006882"/>
        <obo:IAO_0000115>A protected area in Afghanistan.</obo:IAO_0000115>
        <oboInOwl:hasOBONamespace>GAZ</oboInOwl:hasOBONamespace>
        <oboInOwl:id>GAZ:00076857</oboInOwl:id>
        <rdfs:label>Northwest Afghanistan Game Managed Reserve</rdfs:label>
    </owl:NamedIndividual>
    


    <!-- http://purl.obolibrary.org/obo/GAZ_00076858 -->

    <owl:NamedIndividual rdf:about="http://purl.obolibrary.org/obo/GAZ_00076858">
        <obo:RO_0001025 rdf:resource="http://purl.obolibrary.org/obo/GAZ_00006882"/>
        <obo:IAO_0000115>A protected area in Afghanistan.</obo:IAO_0000115>
        <oboInOwl:hasOBONamespace>GAZ</oboInOwl:hasOBONamespace>
        <oboInOwl:id>GAZ:00076858</oboInOwl:id>
        <rdfs:label>Registan Desert Wildlife Managed Reserve</rdfs:label>
    </owl:NamedIndividual>
    


    <!-- http://purl.obolibrary.org/obo/GAZ_00076859 -->

    <owl:NamedIndividual rdf:about="http://purl.obolibrary.org/obo/GAZ_00076859">
        <obo:RO_0001025 rdf:resource="http://purl.obolibrary.org/obo/GAZ_00010626"/>
        <obo:IAO_0000115>A protected area in Afghanistan. Located in southwestern Afghanistan on the border with Iran, 100 km south-southwest of Farah, Nimroz Province.</obo:IAO_0000115>
        <oboInOwl:hasOBONamespace>GAZ</oboInOwl:hasOBONamespace>
        <oboInOwl:id>GAZ:00076859</oboInOwl:id>
        <rdfs:label>Hamun-i-Puzak Waterfowl Sanctuary</rdfs:label>
    </owl:NamedIndividual>
    


    <!-- http://purl.obolibrary.org/obo/GAZ_00076860 -->

    <owl:NamedIndividual rdf:about="http://purl.obolibrary.org/obo/GAZ_00076860">
        <obo:RO_0001025 rdf:resource="http://purl.obolibrary.org/obo/GAZ_00021617"/>
        <obo:IAO_0000115>A protected area in Afghanistan. Located in the southeastern outskirts of Kabul, just south of the Kabul to Gardez highway, Kabul Province.</obo:IAO_0000115>
        <oboInOwl:hasOBONamespace>GAZ</oboInOwl:hasOBONamespace>
        <oboInOwl:id>GAZ:00076860</oboInOwl:id>
        <rdfs:label>Kole Hashmat Khan Waterfowl Sanctuary</rdfs:label>
    </owl:NamedIndividual>
    


    <!-- http://purl.obolibrary.org/obo/GAZ_00076861 -->

    <owl:NamedIndividual rdf:about="http://purl.obolibrary.org/obo/GAZ_00076861">
        <obo:RO_0001025 rdf:resource="http://purl.obolibrary.org/obo/GAZ_00006882"/>
        <obo:IAO_0000115>A protected area in Afghanistan.</obo:IAO_0000115>
        <oboInOwl:hasOBONamespace>GAZ</oboInOwl:hasOBONamespace>
        <oboInOwl:id>GAZ:00076861</oboInOwl:id>
        <rdfs:label>Pamir-i-Buzurg Wildlife Reserve</rdfs:label>
    </owl:NamedIndividual>
    


    <!-- http://purl.obolibrary.org/obo/GAZ_00098853 -->

    <owl:NamedIndividual rdf:about="http://purl.obolibrary.org/obo/GAZ_00098853">
        <obo:RO_0001025 rdf:resource="http://purl.obolibrary.org/obo/GAZ_00010651"/>
        <obo:IAO_0000115>A narrow (in some places less than 10 mile wide) corridor in the Wakhan in the Badakhshan province of Afghanistan. It is located in the Pamir mountain region, with Tajikistan to the north, Pakistan and the disputed territory of the Northern Areas of Jammu and Kashmir to the south and China to the east.</obo:IAO_0000115>
        <oboInOwl:hasOBONamespace>GAZ</oboInOwl:hasOBONamespace>
        <oboInOwl:id>GAZ:00098853</oboInOwl:id>
        <rdfs:label>Wakhan Corridor</rdfs:label>
    </owl:NamedIndividual>
    


    <!-- http://purl.obolibrary.org/obo/GAZ_00098854 -->

    <owl:NamedIndividual rdf:about="http://purl.obolibrary.org/obo/GAZ_00098854">
        <rdf:type rdf:resource="http://purl.obolibrary.org/obo/ENVO_00000004"/>
        <obo:RO_0001025 rdf:resource="http://purl.obolibrary.org/obo/GAZ_00010651"/>
        <obo:IAO_0000115>A district of Badakhshan Province in eastern Afghanistan. It was created in 2005 from part of Khwahan District.</obo:IAO_0000115>
        <oboInOwl:hasOBONamespace>GAZ</oboInOwl:hasOBONamespace>
        <oboInOwl:id>GAZ:00098854</oboInOwl:id>
        <rdfs:label>Kuf Ab District</rdfs:label>
    </owl:NamedIndividual>
    


    <!-- http://purl.obolibrary.org/obo/GAZ_00098855 -->

    <owl:NamedIndividual rdf:about="http://purl.obolibrary.org/obo/GAZ_00098855">
        <rdf:type rdf:resource="http://purl.obolibrary.org/obo/ENVO_00000004"/>
        <obo:RO_0001025 rdf:resource="http://purl.obolibrary.org/obo/GAZ_00010651"/>
        <obo:IAO_0000115>A district in Badakhshan Province, Afghanistan. It was created in 2005 from part of Yaftali Sufla District, itself formed from the Fayzabad District.</obo:IAO_0000115>
        <oboInOwl:hasOBONamespace>GAZ</oboInOwl:hasOBONamespace>
        <oboInOwl:id>GAZ:00098855</oboInOwl:id>
        <rdfs:label>Arghanj Khwa District</rdfs:label>
    </owl:NamedIndividual>
    


    <!-- http://purl.obolibrary.org/obo/GAZ_00098856 -->

    <owl:NamedIndividual rdf:about="http://purl.obolibrary.org/obo/GAZ_00098856">
        <rdf:type rdf:resource="http://purl.obolibrary.org/obo/ENVO_00000004"/>
        <obo:RO_0001025 rdf:resource="http://purl.obolibrary.org/obo/GAZ_00010651"/>
        <obo:IAO_0000115>A district of Badakhshan Province in eastern Afghanistan. The district was formed in 2005 from part of the Baharak District.</obo:IAO_0000115>
        <oboInOwl:hasOBONamespace>GAZ</oboInOwl:hasOBONamespace>
        <oboInOwl:id>GAZ:00098856</oboInOwl:id>
        <rdfs:label>Shuhada District</rdfs:label>
    </owl:NamedIndividual>
    


    <!-- http://purl.obolibrary.org/obo/GAZ_00098857 -->

    <owl:NamedIndividual rdf:about="http://purl.obolibrary.org/obo/GAZ_00098857">
        <rdf:type rdf:resource="http://purl.obolibrary.org/obo/ENVO_00000004"/>
        <obo:RO_0001025 rdf:resource="http://purl.obolibrary.org/obo/GAZ_00010651"/>
        <obo:IAO_0000115>A district of Badakhshan Province in eastern Afghanistan. It was created in 2005 from part of Baharak District.</obo:IAO_0000115>
        <oboInOwl:hasOBONamespace>GAZ</oboInOwl:hasOBONamespace>
        <oboInOwl:id>GAZ:00098857</oboInOwl:id>
        <rdfs:label>Kohistan District</rdfs:label>
    </owl:NamedIndividual>
    


    <!-- http://purl.obolibrary.org/obo/GAZ_00098858 -->

    <owl:NamedIndividual rdf:about="http://purl.obolibrary.org/obo/GAZ_00098858">
        <rdf:type rdf:resource="http://purl.obolibrary.org/obo/ENVO_00000004"/>
        <obo:RO_0001025 rdf:resource="http://purl.obolibrary.org/obo/GAZ_00010651"/>
        <obo:IAO_0000115>A district in Badakhshan Province, Afghanistan. It was created in 2005 from part of Darwaz District.</obo:IAO_0000115>
        <oboInOwl:hasOBONamespace>GAZ</oboInOwl:hasOBONamespace>
        <oboInOwl:id>GAZ:00098858</oboInOwl:id>
        <rdfs:label>Darwazi Bala District</rdfs:label>
    </owl:NamedIndividual>
    


    <!-- http://purl.obolibrary.org/obo/GAZ_00098859 -->

    <owl:NamedIndividual rdf:about="http://purl.obolibrary.org/obo/GAZ_00098859">
        <rdf:type rdf:resource="http://purl.obolibrary.org/obo/ENVO_00000004"/>
        <obo:RO_0001025 rdf:resource="http://purl.obolibrary.org/obo/GAZ_00010651"/>
        <obo:IAO_0000115>A district of Badakhshan Province in eastern Afghanistan. It was created in 2005 from part of Fayzabad District.</obo:IAO_0000115>
        <oboInOwl:hasOBONamespace>GAZ</oboInOwl:hasOBONamespace>
        <oboInOwl:id>GAZ:00098859</oboInOwl:id>
        <rdfs:label>Shiki District</rdfs:label>
    </owl:NamedIndividual>
    


    <!-- http://purl.obolibrary.org/obo/GAZ_00098860 -->

    <owl:NamedIndividual rdf:about="http://purl.obolibrary.org/obo/GAZ_00098860">
        <rdf:type rdf:resource="http://purl.obolibrary.org/obo/ENVO_00000004"/>
        <obo:RO_0001025 rdf:resource="http://purl.obolibrary.org/obo/GAZ_00010651"/>
        <obo:IAO_0000115>A district of Badakhshan Province in Afghanistan. It was created in 2005 from part of Fayzabad District.</obo:IAO_0000115>
        <oboInOwl:hasOBONamespace>GAZ</oboInOwl:hasOBONamespace>
        <oboInOwl:id>GAZ:00098860</oboInOwl:id>
        <rdfs:label>Tagab District</rdfs:label>
    </owl:NamedIndividual>
    


    <!-- http://purl.obolibrary.org/obo/GAZ_00098861 -->

    <owl:NamedIndividual rdf:about="http://purl.obolibrary.org/obo/GAZ_00098861">
        <rdf:type rdf:resource="http://purl.obolibrary.org/obo/ENVO_00000004"/>
        <obo:RO_0001025 rdf:resource="http://purl.obolibrary.org/obo/GAZ_00010651"/>
        <obo:IAO_0000115>A district in Badakhshan Province, Afghanistan. It was created in 2005 from part of Fayzabad District.</obo:IAO_0000115>
        <oboInOwl:hasOBONamespace>GAZ</oboInOwl:hasOBONamespace>
        <oboInOwl:id>GAZ:00098861</oboInOwl:id>
        <rdfs:label>Argo District</rdfs:label>
    </owl:NamedIndividual>
    


    <!-- http://purl.obolibrary.org/obo/GAZ_00098862 -->

    <owl:NamedIndividual rdf:about="http://purl.obolibrary.org/obo/GAZ_00098862">
        <rdf:type rdf:resource="http://purl.obolibrary.org/obo/ENVO_00000004"/>
        <obo:RO_0001025 rdf:resource="http://purl.obolibrary.org/obo/GAZ_00010651"/>
        <obo:IAO_0000115>A district of Badakhshan Province, Afghanistan.</obo:IAO_0000115>
        <oboInOwl:hasOBONamespace>GAZ</oboInOwl:hasOBONamespace>
        <oboInOwl:id>GAZ:00098862</oboInOwl:id>
        <rdfs:label>Khash District</rdfs:label>
    </owl:NamedIndividual>
    


    <!-- http://purl.obolibrary.org/obo/GAZ_00098863 -->

    <owl:NamedIndividual rdf:about="http://purl.obolibrary.org/obo/GAZ_00098863">
        <rdf:type rdf:resource="http://purl.obolibrary.org/obo/ENVO_00000004"/>
        <obo:RO_0001025 rdf:resource="http://purl.obolibrary.org/obo/GAZ_00010651"/>
        <obo:IAO_0000115>A district in Badakhshan Province, Afghanistan. It was created in 2005 from part of Fayzabad District.</obo:IAO_0000115>
        <oboInOwl:hasOBONamespace>GAZ</oboInOwl:hasOBONamespace>
        <oboInOwl:id>GAZ:00098863</oboInOwl:id>
        <rdfs:label>Darayim District</rdfs:label>
    </owl:NamedIndividual>
    


    <!-- http://purl.obolibrary.org/obo/GAZ_00098864 -->

    <owl:NamedIndividual rdf:about="http://purl.obolibrary.org/obo/GAZ_00098864">
        <rdf:type rdf:resource="http://purl.obolibrary.org/obo/ENVO_00000004"/>
        <obo:RO_0001025 rdf:resource="http://purl.obolibrary.org/obo/GAZ_00010651"/>
        <obo:IAO_0000115>A district of Badakhshan Province in eastern Afghanistan. It was created in 2005 from part of Baharak District.</obo:IAO_0000115>
        <oboInOwl:hasOBONamespace>GAZ</oboInOwl:hasOBONamespace>
        <oboInOwl:id>GAZ:00098864</oboInOwl:id>
        <rdfs:label>Yamgan District</rdfs:label>
    </owl:NamedIndividual>
    


    <!-- http://purl.obolibrary.org/obo/GAZ_00098865 -->

    <owl:NamedIndividual rdf:about="http://purl.obolibrary.org/obo/GAZ_00098865">
        <rdf:type rdf:resource="http://purl.obolibrary.org/obo/ENVO_00000004"/>
        <obo:RO_0001025 rdf:resource="http://purl.obolibrary.org/obo/GAZ_00010651"/>
        <obo:IAO_0000115>A district of Badakhshan Province in eastern Afghanistan. It was created in 2005 from part of Fayzabad District.</obo:IAO_0000115>
        <oboInOwl:hasOBONamespace>GAZ</oboInOwl:hasOBONamespace>
        <oboInOwl:id>GAZ:00098865</oboInOwl:id>
        <rdfs:label>Yaftali Sufla District</rdfs:label>
    </owl:NamedIndividual>
    


    <!-- http://purl.obolibrary.org/obo/GAZ_00098866 -->

    <owl:NamedIndividual rdf:about="http://purl.obolibrary.org/obo/GAZ_00098866">
        <rdf:type rdf:resource="http://purl.obolibrary.org/obo/ENVO_00000004"/>
        <obo:RO_0001025 rdf:resource="http://purl.obolibrary.org/obo/GAZ_00010651"/>
        <obo:IAO_0000115>A district of Badakhshan Province in eastern Afghanistan. It was created in 2005 from part of Ragh District.</obo:IAO_0000115>
        <oboInOwl:hasOBONamespace>GAZ</oboInOwl:hasOBONamespace>
        <oboInOwl:id>GAZ:00098866</oboInOwl:id>
        <rdfs:label>Yawan District</rdfs:label>
    </owl:NamedIndividual>
    


    <!-- http://purl.obolibrary.org/obo/GAZ_00098867 -->

    <owl:NamedIndividual rdf:about="http://purl.obolibrary.org/obo/GAZ_00098867">
        <rdf:type rdf:resource="http://purl.obolibrary.org/obo/ENVO_00000004"/>
        <obo:RO_0001025 rdf:resource="http://purl.obolibrary.org/obo/GAZ_00010651"/>
        <obo:IAO_0000115>A district of Badakhshan Province in eastern Afghanistan. It was created in 2005 from part of Kishim District.</obo:IAO_0000115>
        <oboInOwl:hasOBONamespace>GAZ</oboInOwl:hasOBONamespace>
        <oboInOwl:id>GAZ:00098867</oboInOwl:id>
        <rdfs:label>Tishkan District</rdfs:label>
    </owl:NamedIndividual>
    


    <!-- http://purl.obolibrary.org/obo/GAZ_00098868 -->

    <owl:NamedIndividual rdf:about="http://purl.obolibrary.org/obo/GAZ_00098868">
        <rdf:type rdf:resource="http://purl.obolibrary.org/obo/ENVO_00000004"/>
        <obo:RO_0001025 rdf:resource="http://purl.obolibrary.org/obo/GAZ_00010651"/>
        <obo:IAO_0000115>A district of Badakhshan Province in eastern Afghanistan. It was created in 2005 from part of Baharak District.</obo:IAO_0000115>
        <oboInOwl:hasOBONamespace>GAZ</oboInOwl:hasOBONamespace>
        <oboInOwl:id>GAZ:00098868</oboInOwl:id>
        <rdfs:label>Wurduj District</rdfs:label>
    </owl:NamedIndividual>
    


    <!-- http://purl.obolibrary.org/obo/GAZ_00098869 -->

    <owl:NamedIndividual rdf:about="http://purl.obolibrary.org/obo/GAZ_00098869">
        <rdf:type rdf:resource="http://purl.obolibrary.org/obo/ENVO_00000004"/>
        <obo:RO_0001025 rdf:resource="http://purl.obolibrary.org/obo/GAZ_00010659"/>
        <obo:IAO_0000115>A district in Baghlan Province, Afghanistan. It was created in 2005 from part of Andarab District, and is situated in a northeastern direction from Andarab.</obo:IAO_0000115>
        <oboInOwl:hasOBONamespace>GAZ</oboInOwl:hasOBONamespace>
        <oboInOwl:id>GAZ:00098869</oboInOwl:id>
        <rdfs:label>Dih Salah District</rdfs:label>
    </owl:NamedIndividual>
    


    <!-- http://purl.obolibrary.org/obo/GAZ_00098870 -->

    <owl:NamedIndividual rdf:about="http://purl.obolibrary.org/obo/GAZ_00098870">
        <rdf:type rdf:resource="http://purl.obolibrary.org/obo/ENVO_00000004"/>
        <obo:RO_0001025 rdf:resource="http://purl.obolibrary.org/obo/GAZ_00010659"/>
        <obo:IAO_0000115>A district in Baghlan Province, Afghanistan. It was created in 2005 from part of Khost wa Fereng District.</obo:IAO_0000115>
        <oboInOwl:hasOBONamespace>GAZ</oboInOwl:hasOBONamespace>
        <oboInOwl:id>GAZ:00098870</oboInOwl:id>
        <rdfs:label>Farang wa Gharu District</rdfs:label>
    </owl:NamedIndividual>
    


    <!-- http://purl.obolibrary.org/obo/GAZ_00098871 -->

    <owl:NamedIndividual rdf:about="http://purl.obolibrary.org/obo/GAZ_00098871">
        <rdf:type rdf:resource="http://purl.obolibrary.org/obo/ENVO_00000004"/>
        <obo:RO_0001025 rdf:resource="http://purl.obolibrary.org/obo/GAZ_00010659"/>
        <obo:IAO_0000115>A district in Baghlan Province, Afghanistan. It was created in 2005 from part of Khost wa Firing District.</obo:IAO_0000115>
        <oboInOwl:hasOBONamespace>GAZ</oboInOwl:hasOBONamespace>
        <oboInOwl:id>GAZ:00098871</oboInOwl:id>
        <rdfs:label>Guzargahi Nur District</rdfs:label>
    </owl:NamedIndividual>
    


    <!-- http://purl.obolibrary.org/obo/GAZ_00098872 -->

    <owl:NamedIndividual rdf:about="http://purl.obolibrary.org/obo/GAZ_00098872">
        <rdf:type rdf:resource="http://purl.obolibrary.org/obo/ENVO_00000004"/>
        <obo:RO_0001025 rdf:resource="http://purl.obolibrary.org/obo/GAZ_00010659"/>
        <obo:IAO_0000115>A district in Baghlan Province, Afghanistan. It was created in 2005 from part of Andarab District.</obo:IAO_0000115>
        <oboInOwl:hasOBONamespace>GAZ</oboInOwl:hasOBONamespace>
        <oboInOwl:id>GAZ:00098872</oboInOwl:id>
        <rdfs:label>Jelga District</rdfs:label>
    </owl:NamedIndividual>
    


    <!-- http://purl.obolibrary.org/obo/GAZ_00098873 -->

    <owl:NamedIndividual rdf:about="http://purl.obolibrary.org/obo/GAZ_00098873">
        <rdf:type rdf:resource="http://purl.obolibrary.org/obo/ENVO_00000004"/>
        <obo:RO_0001025 rdf:resource="http://purl.obolibrary.org/obo/GAZ_00010659"/>
        <obo:IAO_0000115>A district in Baghlan Province, Afghanistan. It was created in 2005 from part of Andarab District.</obo:IAO_0000115>
        <oboInOwl:hasOBONamespace>GAZ</oboInOwl:hasOBONamespace>
        <oboInOwl:id>GAZ:00098873</oboInOwl:id>
        <rdfs:label>Puli Hisar District</rdfs:label>
    </owl:NamedIndividual>
    


    <!-- http://purl.obolibrary.org/obo/GAZ_00098874 -->

    <owl:NamedIndividual rdf:about="http://purl.obolibrary.org/obo/GAZ_00098874">
        <rdf:type rdf:resource="http://purl.obolibrary.org/obo/ENVO_00000004"/>
        <obo:RO_0001025 rdf:resource="http://purl.obolibrary.org/obo/GAZ_00010654"/>
        <obo:IAO_0000115>A district in Balkh Province, Afghanistan. It was created in 2005 from part of Kishindih District.</obo:IAO_0000115>
        <oboInOwl:hasOBONamespace>GAZ</oboInOwl:hasOBONamespace>
        <oboInOwl:id>GAZ:00098874</oboInOwl:id>
        <rdfs:label>Zari District</rdfs:label>
    </owl:NamedIndividual>
    


    <!-- http://purl.obolibrary.org/obo/GAZ_00098875 -->

    <owl:NamedIndividual rdf:about="http://purl.obolibrary.org/obo/GAZ_00098875">
        <rdf:type rdf:resource="http://purl.obolibrary.org/obo/ENVO_00000004"/>
        <obo:RO_0001025 rdf:resource="http://purl.obolibrary.org/obo/GAZ_00010657"/>
        <obo:IAO_0000115>A district in Bamyan Province, Afghanistan. It was created in 2005 from part of Kahmard District, and until 2004 was part of Baghlan Province.</obo:IAO_0000115>
        <oboInOwl:hasOBONamespace>GAZ</oboInOwl:hasOBONamespace>
        <oboInOwl:id>GAZ:00098875</oboInOwl:id>
        <rdfs:label>Sayghan District</rdfs:label>
    </owl:NamedIndividual>
    


    <!-- http://purl.obolibrary.org/obo/GAZ_00098876 -->

    <owl:NamedIndividual rdf:about="http://purl.obolibrary.org/obo/GAZ_00098876">
        <rdf:type rdf:resource="http://purl.obolibrary.org/obo/ENVO_00000004"/>
        <obo:RO_0001025 rdf:resource="http://purl.obolibrary.org/obo/GAZ_00010656"/>
        <obo:IAO_0000115>A district in Daykundi Province, Afghanistan. It was created in 2005 from the Daykundi district.</obo:IAO_0000115>
        <oboInOwl:hasOBONamespace>GAZ</oboInOwl:hasOBONamespace>
        <oboInOwl:id>GAZ:00098876</oboInOwl:id>
        <rdfs:label>Khadir District</rdfs:label>
    </owl:NamedIndividual>
    


    <!-- http://purl.obolibrary.org/obo/GAZ_00098877 -->

    <owl:NamedIndividual rdf:about="http://purl.obolibrary.org/obo/GAZ_00098877">
        <obo:RO_0001025 rdf:resource="http://purl.obolibrary.org/obo/GAZ_00010656"/>
        <oboInOwl:hasOBONamespace>GAZ</oboInOwl:hasOBONamespace>
        <oboInOwl:id>GAZ:00098877</oboInOwl:id>
        <rdfs:label>Kiti District</rdfs:label>
    </owl:NamedIndividual>
    


    <!-- http://purl.obolibrary.org/obo/GAZ_00098878 -->

    <owl:NamedIndividual rdf:about="http://purl.obolibrary.org/obo/GAZ_00098878">
        <rdf:type rdf:resource="http://purl.obolibrary.org/obo/ENVO_00000004"/>
        <obo:RO_0001025 rdf:resource="http://purl.obolibrary.org/obo/GAZ_00010656"/>
        <obo:IAO_0000115>A district in Daykundi Province, Afghanistan. It was created in 2005 from Shahristan district.</obo:IAO_0000115>
        <oboInOwl:hasOBONamespace>GAZ</oboInOwl:hasOBONamespace>
        <oboInOwl:id>GAZ:00098878</oboInOwl:id>
        <rdfs:label>Miramor District</rdfs:label>
    </owl:NamedIndividual>
    


    <!-- http://purl.obolibrary.org/obo/GAZ_00098879 -->

    <owl:NamedIndividual rdf:about="http://purl.obolibrary.org/obo/GAZ_00098879">
        <rdf:type rdf:resource="http://purl.obolibrary.org/obo/ENVO_00000004"/>
        <obo:RO_0001025 rdf:resource="http://purl.obolibrary.org/obo/GAZ_00010656"/>
        <obo:IAO_0000115>A district in Daykundi Province, Afghanistan. It was created in 2005 from Daykundi district.</obo:IAO_0000115>
        <oboInOwl:hasOBONamespace>GAZ</oboInOwl:hasOBONamespace>
        <oboInOwl:id>GAZ:00098879</oboInOwl:id>
        <rdfs:label>Nili District</rdfs:label>
    </owl:NamedIndividual>
    


    <!-- http://purl.obolibrary.org/obo/GAZ_00098880 -->

    <owl:NamedIndividual rdf:about="http://purl.obolibrary.org/obo/GAZ_00098880">
        <rdf:type rdf:resource="http://purl.obolibrary.org/obo/ENVO_00000004"/>
        <obo:RO_0001025 rdf:resource="http://purl.obolibrary.org/obo/GAZ_00010656"/>
        <obo:IAO_0000115>A district in Daykundi Province, Afghanistan. It was created in 2005 from Daykundi district.</obo:IAO_0000115>
        <oboInOwl:hasOBONamespace>GAZ</oboInOwl:hasOBONamespace>
        <oboInOwl:id>GAZ:00098880</oboInOwl:id>
        <rdfs:label>Sangi Takht District</rdfs:label>
    </owl:NamedIndividual>
    


    <!-- http://purl.obolibrary.org/obo/GAZ_00098881 -->

    <owl:NamedIndividual rdf:about="http://purl.obolibrary.org/obo/GAZ_00098881">
        <rdf:type rdf:resource="http://purl.obolibrary.org/obo/ENVO_00000004"/>
        <obo:RO_0001025 rdf:resource="http://purl.obolibrary.org/obo/GAZ_00010656"/>
        <obo:IAO_0000115>A district in Daykundi Province, Afghanistan.</obo:IAO_0000115>
        <oboInOwl:hasOBONamespace>GAZ</oboInOwl:hasOBONamespace>
        <oboInOwl:id>GAZ:00098881</oboInOwl:id>
        <rdfs:label>Ashtarlai District</rdfs:label>
    </owl:NamedIndividual>
    


    <!-- http://purl.obolibrary.org/obo/GAZ_00098882 -->

    <owl:NamedIndividual rdf:about="http://purl.obolibrary.org/obo/GAZ_00098882">
        <rdf:type rdf:resource="http://purl.obolibrary.org/obo/ENVO_00000004"/>
        <obo:RO_0001025 rdf:resource="http://purl.obolibrary.org/obo/GAZ_00010648"/>
        <obo:IAO_0000115>A district in Faryab Province, Afghanistan. It was created in 2005 from part of Bilchiragh District.</obo:IAO_0000115>
        <oboInOwl:hasOBONamespace>GAZ</oboInOwl:hasOBONamespace>
        <oboInOwl:id>GAZ:00098882</oboInOwl:id>
        <rdfs:label>Gurziwan District</rdfs:label>
    </owl:NamedIndividual>
    


    <!-- http://purl.obolibrary.org/obo/GAZ_00098883 -->

    <owl:NamedIndividual rdf:about="http://purl.obolibrary.org/obo/GAZ_00098883">
        <rdf:type rdf:resource="http://purl.obolibrary.org/obo/ENVO_00000004"/>
        <obo:RO_0001025 rdf:resource="http://purl.obolibrary.org/obo/GAZ_00010648"/>
        <obo:IAO_0000115>A district in Faryab Province, Afghanistan. It was created in 2005 from the western part of Andkhoy District.</obo:IAO_0000115>
        <oboInOwl:hasOBONamespace>GAZ</oboInOwl:hasOBONamespace>
        <oboInOwl:id>GAZ:00098883</oboInOwl:id>
        <rdfs:label>Qurghan District</rdfs:label>
    </owl:NamedIndividual>
    


    <!-- http://purl.obolibrary.org/obo/GAZ_00098884 -->

    <owl:NamedIndividual rdf:about="http://purl.obolibrary.org/obo/GAZ_00098884">
        <rdf:type rdf:resource="http://purl.obolibrary.org/obo/ENVO_00000004"/>
        <obo:RO_0001025 rdf:resource="http://purl.obolibrary.org/obo/GAZ_00010652"/>
        <obo:IAO_0000115>A district in Ghazni Province, Afghanistan. It was created in 2005 from the large Bahrami Shahid District.</obo:IAO_0000115>
        <oboInOwl:hasOBONamespace>GAZ</oboInOwl:hasOBONamespace>
        <oboInOwl:id>GAZ:00098884</oboInOwl:id>
        <rdfs:label>Khwaja Umari District</rdfs:label>
    </owl:NamedIndividual>
    


    <!-- http://purl.obolibrary.org/obo/GAZ_00098885 -->

    <owl:NamedIndividual rdf:about="http://purl.obolibrary.org/obo/GAZ_00098885">
        <rdf:type rdf:resource="http://purl.obolibrary.org/obo/ENVO_00000004"/>
        <obo:RO_0001025 rdf:resource="http://purl.obolibrary.org/obo/GAZ_00010652"/>
        <obo:IAO_0000115>A district in Ghazni Province, Afghanistan. It was previously part of Jaghatu District. To the east it is surrounded by Ghazni City District, to the south by Waghaz District, to the west by Jaghatu District, to the north by the Rashidan district and to the Northeast by Khwaja Umari district.</obo:IAO_0000115>
        <oboInOwl:hasOBONamespace>GAZ</oboInOwl:hasOBONamespace>
        <oboInOwl:id>GAZ:00098885</oboInOwl:id>
        <rdfs:label>Khugiani District</rdfs:label>
    </owl:NamedIndividual>
    


    <!-- http://purl.obolibrary.org/obo/GAZ_00098886 -->

    <owl:NamedIndividual rdf:about="http://purl.obolibrary.org/obo/GAZ_00098886">
        <rdf:type rdf:resource="http://purl.obolibrary.org/obo/ENVO_00000004"/>
        <obo:RO_0001025 rdf:resource="http://purl.obolibrary.org/obo/GAZ_00010652"/>
        <obo:IAO_0000115>A district in Ghazni Province, Afghanistan. It was formed in 2005 from part of Muqur District.</obo:IAO_0000115>
        <oboInOwl:hasOBONamespace>GAZ</oboInOwl:hasOBONamespace>
        <oboInOwl:id>GAZ:00098886</oboInOwl:id>
        <rdfs:label>Waghaz District</rdfs:label>
    </owl:NamedIndividual>
    


    <!-- http://purl.obolibrary.org/obo/GAZ_00098887 -->

    <owl:NamedIndividual rdf:about="http://purl.obolibrary.org/obo/GAZ_00098887">
        <rdf:type rdf:resource="http://purl.obolibrary.org/obo/ENVO_00000004"/>
        <obo:RO_0001025 rdf:resource="http://purl.obolibrary.org/obo/GAZ_00010652"/>
        <obo:IAO_0000115>A district in Afghanistan; it was created from the larger Jaghatu district.</obo:IAO_0000115>
        <oboInOwl:hasOBONamespace>GAZ</oboInOwl:hasOBONamespace>
        <oboInOwl:id>GAZ:00098887</oboInOwl:id>
        <rdfs:label>Rashidan District</rdfs:label>
    </owl:NamedIndividual>
    


    <!-- http://purl.obolibrary.org/obo/GAZ_00098888 -->

    <owl:NamedIndividual rdf:about="http://purl.obolibrary.org/obo/GAZ_00098888">
        <rdf:type rdf:resource="http://purl.obolibrary.org/obo/ENVO_00000004"/>
        <obo:RO_0001025 rdf:resource="http://purl.obolibrary.org/obo/GAZ_00010649"/>
        <obo:IAO_0000115>A district of Ghor Province, Afghanistan. It was created from the northwestern part of Chaghcharan District.</obo:IAO_0000115>
        <oboInOwl:hasOBONamespace>GAZ</oboInOwl:hasOBONamespace>
        <oboInOwl:id>GAZ:00098888</oboInOwl:id>
        <rdfs:label>Charsada District</rdfs:label>
    </owl:NamedIndividual>
    


    <!-- http://purl.obolibrary.org/obo/GAZ_00098889 -->

    <owl:NamedIndividual rdf:about="http://purl.obolibrary.org/obo/GAZ_00098889">
        <rdf:type rdf:resource="http://purl.obolibrary.org/obo/ENVO_00000004"/>
        <obo:RO_0001025 rdf:resource="http://purl.obolibrary.org/obo/GAZ_00010649"/>
        <obo:IAO_0000115>A district in Ghor Province, Afghanistan. It was created in 2005 from the southeastern part of Chaghcharan District.</obo:IAO_0000115>
        <oboInOwl:hasOBONamespace>GAZ</oboInOwl:hasOBONamespace>
        <oboInOwl:id>GAZ:00098889</oboInOwl:id>
        <rdfs:label>Dawlat Yar District</rdfs:label>
    </owl:NamedIndividual>
    


    <!-- http://purl.obolibrary.org/obo/GAZ_00098890 -->

    <owl:NamedIndividual rdf:about="http://purl.obolibrary.org/obo/GAZ_00098890">
        <rdf:type rdf:resource="http://purl.obolibrary.org/obo/ENVO_00000004"/>
        <obo:RO_0001025 rdf:resource="http://purl.obolibrary.org/obo/GAZ_00010649"/>
        <obo:IAO_0000115>A district in Ghor Province, Afghanistan. It was created from part of the much larger Chaghcharan District.</obo:IAO_0000115>
        <oboInOwl:hasOBONamespace>GAZ</oboInOwl:hasOBONamespace>
        <oboInOwl:id>GAZ:00098890</oboInOwl:id>
        <rdfs:label>Du Layna District</rdfs:label>
    </owl:NamedIndividual>
    


    <!-- http://purl.obolibrary.org/obo/GAZ_00098891 -->

    <owl:NamedIndividual rdf:about="http://purl.obolibrary.org/obo/GAZ_00098891">
        <obo:RO_0001025 rdf:resource="http://purl.obolibrary.org/obo/GAZ_00010650"/>
        <obo:IAO_0000115>A district in Helmand Province, Afghanistan.</obo:IAO_0000115>
        <oboInOwl:hasOBONamespace>GAZ</oboInOwl:hasOBONamespace>
        <oboInOwl:id>GAZ:00098891</oboInOwl:id>
        <rdfs:label>Gerishk District</rdfs:label>
    </owl:NamedIndividual>
    


    <!-- http://purl.obolibrary.org/obo/GAZ_00098892 -->

    <owl:NamedIndividual rdf:about="http://purl.obolibrary.org/obo/GAZ_00098892">
        <obo:RO_0001025 rdf:resource="http://purl.obolibrary.org/obo/GAZ_00010650"/>
        <obo:IAO_0000115>A district situated in the Southeastern part of Helmand Province, Afghanistan along the W bank of the Helmand River.</obo:IAO_0000115>
        <oboInOwl:hasOBONamespace>GAZ</oboInOwl:hasOBONamespace>
        <oboInOwl:id>GAZ:00098892</oboInOwl:id>
        <rdfs:label>Khanashin District</rdfs:label>
    </owl:NamedIndividual>
    


    <!-- http://purl.obolibrary.org/obo/GAZ_00098893 -->

    <owl:NamedIndividual rdf:about="http://purl.obolibrary.org/obo/GAZ_00098893">
        <obo:RO_0001025 rdf:resource="http://purl.obolibrary.org/obo/GAZ_00021589"/>
        <obo:IAO_0000115>A populated place. A city in western Afghanistan. It is situated in the valley of the Hari River, which flows from the mountains of central Afghanistan to the Karakum Desert in Turkmenistan.</obo:IAO_0000115>
        <oboInOwl:hasOBONamespace>GAZ</oboInOwl:hasOBONamespace>
        <oboInOwl:id>GAZ:00098893</oboInOwl:id>
        <rdfs:label>Herat</rdfs:label>
    </owl:NamedIndividual>
    


    <!-- http://purl.obolibrary.org/obo/GAZ_00098894 -->

    <owl:NamedIndividual rdf:about="http://purl.obolibrary.org/obo/GAZ_00098894">
        <rdf:type rdf:resource="http://purl.obolibrary.org/obo/ENVO_00000004"/>
        <obo:RO_0001025 rdf:resource="http://purl.obolibrary.org/obo/GAZ_00010635"/>
        <obo:IAO_0000115>A district of Kabul province in Afghanistan. In 1991-01, Farza was separated as an independent district from Mir Bacha Kot District.</obo:IAO_0000115>
        <oboInOwl:hasOBONamespace>GAZ</oboInOwl:hasOBONamespace>
        <oboInOwl:id>GAZ:00098894</oboInOwl:id>
        <rdfs:label>Farza District</rdfs:label>
    </owl:NamedIndividual>
    


    <!-- http://purl.obolibrary.org/obo/GAZ_00098895 -->

    <owl:NamedIndividual rdf:about="http://purl.obolibrary.org/obo/GAZ_00098895">
        <obo:RO_0001025 rdf:resource="http://purl.obolibrary.org/obo/GAZ_00021617"/>
        <obo:IAO_0000115>The capital and largest city of Afghanistan.</obo:IAO_0000115>
        <oboInOwl:hasOBONamespace>GAZ</oboInOwl:hasOBONamespace>
        <oboInOwl:id>GAZ:00098895</oboInOwl:id>
        <rdfs:label>Kabul</rdfs:label>
    </owl:NamedIndividual>
    


    <!-- http://purl.obolibrary.org/obo/GAZ_00098896 -->

    <owl:NamedIndividual rdf:about="http://purl.obolibrary.org/obo/GAZ_00098896">
        <obo:RO_0001025 rdf:resource="http://purl.obolibrary.org/obo/GAZ_00021637"/>
        <obo:IAO_0000115>The second largest city in Afghanistan, the capital of Kandahar Province.</obo:IAO_0000115>
        <oboInOwl:hasOBONamespace>GAZ</oboInOwl:hasOBONamespace>
        <oboInOwl:id>GAZ:00098896</oboInOwl:id>
        <rdfs:label>Kandahar</rdfs:label>
    </owl:NamedIndividual>
    


    <!-- http://purl.obolibrary.org/obo/GAZ_00098897 -->

    <owl:NamedIndividual rdf:about="http://purl.obolibrary.org/obo/GAZ_00098897">
        <rdf:type rdf:resource="http://purl.obolibrary.org/obo/ENVO_00000004"/>
        <obo:RO_0001025 rdf:resource="http://purl.obolibrary.org/obo/GAZ_00010642"/>
        <obo:IAO_0000115>A district of Kandahar District, Afghanistan, created in 2005. It was in the northern part of Shah Wali Kot District.</obo:IAO_0000115>
        <oboInOwl:hasOBONamespace>GAZ</oboInOwl:hasOBONamespace>
        <oboInOwl:id>GAZ:00098897</oboInOwl:id>
        <rdfs:label>Miyannasheen District</rdfs:label>
    </owl:NamedIndividual>
    


    <!-- http://purl.obolibrary.org/obo/GAZ_00098898 -->

    <owl:NamedIndividual rdf:about="http://purl.obolibrary.org/obo/GAZ_00098898">
        <rdf:type rdf:resource="http://purl.obolibrary.org/obo/ENVO_00000004"/>
        <obo:RO_0001025 rdf:resource="http://purl.obolibrary.org/obo/GAZ_00010642"/>
        <obo:IAO_0000115>A district in the northern part of Kandahar Province, shifted from Oruzgan Province, Afghanistan. It borders Oruzgan Province to the west, north and east and Shah Wali Kot, Khakrez and Ghorak districts to the south.</obo:IAO_0000115>
        <oboInOwl:hasOBONamespace>GAZ</oboInOwl:hasOBONamespace>
        <oboInOwl:id>GAZ:00098898</oboInOwl:id>
        <rdfs:label>Naish District</rdfs:label>
    </owl:NamedIndividual>
    


    <!-- http://purl.obolibrary.org/obo/GAZ_00098899 -->

    <owl:NamedIndividual rdf:about="http://purl.obolibrary.org/obo/GAZ_00098899">
        <obo:RO_0001025 rdf:resource="http://purl.obolibrary.org/obo/GAZ_00010637"/>
        <obo:IAO_0000115>A district, created from the of split bigger Kohistan District in Kapisa Province, Afghanistan in its southern part. The center is to be the village of Keshektan.</obo:IAO_0000115>
        <oboInOwl:hasOBONamespace>GAZ</oboInOwl:hasOBONamespace>
        <oboInOwl:id>GAZ:00098899</oboInOwl:id>
        <rdfs:label>Hesa Duwum Kohistan District</rdfs:label>
    </owl:NamedIndividual>
    


    <!-- http://purl.obolibrary.org/obo/GAZ_00098900 -->

    <owl:NamedIndividual rdf:about="http://purl.obolibrary.org/obo/GAZ_00098900">
        <obo:RO_0001025 rdf:resource="http://purl.obolibrary.org/obo/GAZ_00010637"/>
        <obo:IAO_0000115>A district created from the split bigger Kohistan District in Kapisa Province, Afghanistan. The district center is Kohistan.</obo:IAO_0000115>
        <oboInOwl:hasOBONamespace>GAZ</oboInOwl:hasOBONamespace>
        <oboInOwl:id>GAZ:00098900</oboInOwl:id>
        <rdfs:label>Kohistan Hesa Awal District</rdfs:label>
    </owl:NamedIndividual>
    


    <!-- http://purl.obolibrary.org/obo/GAZ_00098901 -->

    <owl:NamedIndividual rdf:about="http://purl.obolibrary.org/obo/GAZ_00098901">
        <obo:RO_0001025 rdf:resource="http://purl.obolibrary.org/obo/GAZ_00010634"/>
        <obo:IAO_0000115>A district situated in the western part of Khost Province, Afghanistan. It borders with Paktia Province to the West, Nadir Shah Kot District to the East and Spera District to the South.</obo:IAO_0000115>
        <oboInOwl:hasOBONamespace>GAZ</oboInOwl:hasOBONamespace>
        <oboInOwl:id>GAZ:00098901</oboInOwl:id>
        <rdfs:label>Shamal District</rdfs:label>
    </owl:NamedIndividual>
    


    <!-- http://purl.obolibrary.org/obo/GAZ_00098902 -->

    <owl:NamedIndividual rdf:about="http://purl.obolibrary.org/obo/GAZ_00098902">
        <obo:RO_0001025 rdf:resource="http://purl.obolibrary.org/obo/GAZ_00021529"/>
        <obo:IAO_0000115>A populated place. A city in Yakawlang District, Bamyan Province, Afghanistan. It is the capital of Yakawlang District.</obo:IAO_0000115>
        <oboInOwl:hasOBONamespace>GAZ</oboInOwl:hasOBONamespace>
        <oboInOwl:id>GAZ:00098902</oboInOwl:id>
        <rdfs:label>Yakawlang</rdfs:label>
    </owl:NamedIndividual>
    


    <!-- http://purl.obolibrary.org/obo/GAZ_00098903 -->

    <owl:NamedIndividual rdf:about="http://purl.obolibrary.org/obo/GAZ_00098903">
        <obo:RO_0001025 rdf:resource="http://purl.obolibrary.org/obo/GAZ_00010632"/>
        <obo:IAO_0000115>A district located in the western-central part of Kunar Province, Afghanistan, 30 km West from Asadabad.</obo:IAO_0000115>
        <oboInOwl:hasOBONamespace>GAZ</oboInOwl:hasOBONamespace>
        <oboInOwl:id>GAZ:00098903</oboInOwl:id>
        <rdfs:label>Dara-I-Pech district</rdfs:label>
    </owl:NamedIndividual>
    


    <!-- http://purl.obolibrary.org/obo/GAZ_00098904 -->

    <owl:NamedIndividual rdf:about="http://purl.obolibrary.org/obo/GAZ_00098904">
        <obo:RO_0001025 rdf:resource="http://purl.obolibrary.org/obo/GAZ_00010632"/>
        <obo:IAO_0000115>A district situated in the western part of Kunar Province, Afghanistan and was part of Nurgal district. It borders with Nangarhar Province to the west, Chapa Dara district to the north, Chawkay district to the east and Nurgal district to the south.</obo:IAO_0000115>
        <oboInOwl:hasOBONamespace>GAZ</oboInOwl:hasOBONamespace>
        <oboInOwl:id>GAZ:00098904</oboInOwl:id>
        <rdfs:label>Ghaziabad district</rdfs:label>
    </owl:NamedIndividual>
    


    <!-- http://purl.obolibrary.org/obo/GAZ_00098905 -->

    <owl:NamedIndividual rdf:about="http://purl.obolibrary.org/obo/GAZ_00098905">
        <rdf:type rdf:resource="http://purl.obolibrary.org/obo/ENVO_00000004"/>
        <obo:RO_0001025 rdf:resource="http://purl.obolibrary.org/obo/GAZ_00010632"/>
        <obo:IAO_0000115>A district in Kunar Province, Afghanistan. It was split from Chapa Dara district.</obo:IAO_0000115>
        <oboInOwl:hasOBONamespace>GAZ</oboInOwl:hasOBONamespace>
        <oboInOwl:id>GAZ:00098905</oboInOwl:id>
        <rdfs:label>Shaygal Wa Shiltan district</rdfs:label>
    </owl:NamedIndividual>
    


    <!-- http://purl.obolibrary.org/obo/GAZ_00098906 -->

    <owl:NamedIndividual rdf:about="http://purl.obolibrary.org/obo/GAZ_00098906">
        <obo:RO_0001025 rdf:resource="http://purl.obolibrary.org/obo/GAZ_00010632"/>
        <obo:IAO_0000115>A district situated in the central part of Kunar Province, Afghanistan. It was split from Asadabad district.</obo:IAO_0000115>
        <oboInOwl:hasOBONamespace>GAZ</oboInOwl:hasOBONamespace>
        <oboInOwl:id>GAZ:00098906</oboInOwl:id>
        <rdfs:label>Wata Pur District</rdfs:label>
    </owl:NamedIndividual>
    


    <!-- http://purl.obolibrary.org/obo/GAZ_00098907 -->

    <owl:NamedIndividual rdf:about="http://purl.obolibrary.org/obo/GAZ_00098907">
        <rdf:type rdf:resource="http://purl.obolibrary.org/obo/ENVO_00000004"/>
        <obo:RO_0001025 rdf:resource="http://purl.obolibrary.org/obo/GAZ_00010633"/>
        <obo:IAO_0000115>A district in Lowgar Province. Kharwar District has been created from the former big Charkh District.</obo:IAO_0000115>
        <oboInOwl:hasOBONamespace>GAZ</oboInOwl:hasOBONamespace>
        <oboInOwl:id>GAZ:00098907</oboInOwl:id>
        <rdfs:label>Kharwar District</rdfs:label>
    </owl:NamedIndividual>
    


    <!-- http://purl.obolibrary.org/obo/GAZ_00098908 -->

    <owl:NamedIndividual rdf:about="http://purl.obolibrary.org/obo/GAZ_00098908">
        <obo:RO_0001025 rdf:resource="http://purl.obolibrary.org/obo/GAZ_00010633"/>
        <obo:IAO_0000115>A district in Lowgar Province. Was in Paktia Province.</obo:IAO_0000115>
        <oboInOwl:hasOBONamespace>GAZ</oboInOwl:hasOBONamespace>
        <oboInOwl:id>GAZ:00098908</oboInOwl:id>
        <rdfs:label>Azra District</rdfs:label>
    </owl:NamedIndividual>
    


    <!-- http://purl.obolibrary.org/obo/GAZ_00098909 -->

    <owl:NamedIndividual rdf:about="http://purl.obolibrary.org/obo/GAZ_00098909">
        <rdf:type rdf:resource="http://purl.obolibrary.org/obo/ENVO_00000004"/>
        <obo:RO_0001025 rdf:resource="http://purl.obolibrary.org/obo/GAZ_00010631"/>
        <obo:IAO_0000115>A district in Nurestan Province, Afghanistan.</obo:IAO_0000115>
        <oboInOwl:hasOBONamespace>GAZ</oboInOwl:hasOBONamespace>
        <oboInOwl:id>GAZ:00098909</oboInOwl:id>
        <rdfs:label>Doab District</rdfs:label>
    </owl:NamedIndividual>
    


    <!-- http://purl.obolibrary.org/obo/GAZ_00098910 -->

    <owl:NamedIndividual rdf:about="http://purl.obolibrary.org/obo/GAZ_00098910">
        <rdf:type rdf:resource="http://purl.obolibrary.org/obo/ENVO_00000004"/>
        <obo:RO_0001025 rdf:resource="http://purl.obolibrary.org/obo/GAZ_00010631"/>
        <obo:IAO_0000115>A district in Nurestan Province, Afghanistan.</obo:IAO_0000115>
        <oboInOwl:hasOBONamespace>GAZ</oboInOwl:hasOBONamespace>
        <oboInOwl:id>GAZ:00098910</oboInOwl:id>
        <rdfs:label>Nurgram District</rdfs:label>
    </owl:NamedIndividual>
    


    <!-- http://purl.obolibrary.org/obo/GAZ_00098911 -->

    <owl:NamedIndividual rdf:about="http://purl.obolibrary.org/obo/GAZ_00098911">
        <rdf:type rdf:resource="http://purl.obolibrary.org/obo/ENVO_00000004"/>
        <obo:RO_0001025 rdf:resource="http://purl.obolibrary.org/obo/GAZ_00010631"/>
        <obo:IAO_0000115>A district in Nurestan Province, Afghanistan.</obo:IAO_0000115>
        <oboInOwl:hasOBONamespace>GAZ</oboInOwl:hasOBONamespace>
        <oboInOwl:id>GAZ:00098911</oboInOwl:id>
        <rdfs:label>Paruns District</rdfs:label>
    </owl:NamedIndividual>
    


    <!-- http://purl.obolibrary.org/obo/GAZ_00098912 -->

    <owl:NamedIndividual rdf:about="http://purl.obolibrary.org/obo/GAZ_00098912">
        <rdf:type rdf:resource="http://purl.obolibrary.org/obo/ENVO_00000004"/>
        <obo:RO_0001025 rdf:resource="http://purl.obolibrary.org/obo/GAZ_00010646"/>
        <obo:IAO_0000115>A district in Paktia Province, Afghanistan.</obo:IAO_0000115>
        <oboInOwl:hasOBONamespace>GAZ</oboInOwl:hasOBONamespace>
        <oboInOwl:id>GAZ:00098912</oboInOwl:id>
        <rdfs:label>Ahmadzai District</rdfs:label>
    </owl:NamedIndividual>
    


    <!-- http://purl.obolibrary.org/obo/GAZ_00098913 -->

    <owl:NamedIndividual rdf:about="http://purl.obolibrary.org/obo/GAZ_00098913">
        <rdf:type rdf:resource="http://purl.obolibrary.org/obo/ENVO_00000004"/>
        <obo:RO_0001025 rdf:resource="http://purl.obolibrary.org/obo/GAZ_00010646"/>
        <obo:IAO_0000115>A district in Paktia Province, Afghanistan.</obo:IAO_0000115>
        <oboInOwl:hasOBONamespace>GAZ</oboInOwl:hasOBONamespace>
        <oboInOwl:id>GAZ:00098913</oboInOwl:id>
        <rdfs:label>Wuza Zadran District</rdfs:label>
    </owl:NamedIndividual>
    


    <!-- http://purl.obolibrary.org/obo/GAZ_00129987 -->

    <owl:NamedIndividual rdf:about="http://purl.obolibrary.org/obo/GAZ_00129987">
        <obo:RO_0001025 rdf:resource="http://purl.obolibrary.org/obo/GAZ_00011784"/>
        <obo:IAO_0000115>A protected area. It consists of the northern part of the massif of Mount Everest in the southwest corner of the Tibet Autonomous Region in the border region between the Tibetan, China and Nepal biogeographical realms. It extends from the border with Nepal in the south, to the watershed between the Yaluzangbu River and the southern regions of Tibet in the north.</obo:IAO_0000115>
        <oboInOwl:hasOBONamespace>GAZ</oboInOwl:hasOBONamespace>
        <oboInOwl:id>GAZ:00129987</oboInOwl:id>
        <rdfs:label>Qomolangma National Nature Reserve</rdfs:label>
    </owl:NamedIndividual>
    


    <!-- http://purl.obolibrary.org/obo/GAZ_00143916 -->

    <owl:NamedIndividual rdf:about="http://purl.obolibrary.org/obo/GAZ_00143916">
        <obo:RO_0001025 rdf:resource="http://purl.obolibrary.org/obo/GAZ_00004988"/>
        <obo:IAO_0000115>A large glacier in the Pamir Mountains of central Tajikistan. The glacier follows a generally northward path to the east of the 6,595 m Garmo Peak. The glacier begins at an elevation of 6,200 m above sea level, and eventually melts and empties into the Balandkiik River near the border with Kyrgyzstan at an elevation of 2,909 m. Its waters eventually feed into the Muksu, Vakhsh, and Amu Darya rivers.</obo:IAO_0000115>
        <oboInOwl:hasOBONamespace>GAZ</oboInOwl:hasOBONamespace>
        <oboInOwl:id>GAZ:00143916</oboInOwl:id>
        <rdfs:label>Fedchenko Glacier</rdfs:label>
    </owl:NamedIndividual>
    


    <!-- http://purl.obolibrary.org/obo/GAZ_00143917 -->

    <owl:NamedIndividual rdf:about="http://purl.obolibrary.org/obo/GAZ_00143917">
        <obo:RO_0001025 rdf:resource="http://purl.obolibrary.org/obo/GAZ_00004988"/>
        <obo:IAO_0000115>A glacier in the Pamir Mountains, near Qullai Revolutsiya, Gorno-Badakhshan, central Tajikistan.</obo:IAO_0000115>
        <oboInOwl:hasOBONamespace>GAZ</oboInOwl:hasOBONamespace>
        <oboInOwl:id>GAZ:00143917</oboInOwl:id>
        <rdfs:label>Russian Geographical Society Glacier</rdfs:label>
    </owl:NamedIndividual>
    


    <!-- http://purl.obolibrary.org/obo/GAZ_00144828 -->

    <owl:NamedIndividual rdf:about="http://purl.obolibrary.org/obo/GAZ_00144828">
        <obo:RO_0001025 rdf:resource="http://purl.obolibrary.org/obo/GAZ_00004988"/>
        <obo:IAO_0000115>A mountain range in Central Asia, in the western part of the Pamir-Alay system, stretching over 200 km in the general east-west direction across the territory of Tajikistan and Uzbekistan. The Gissar Range lies south of the Zeravshan Range, extending north of Dushanbe through Tajikistan&apos;s Gissar District and reaching Uzbekistan at the north tip of Surkhandarya Province.</obo:IAO_0000115>
        <oboInOwl:hasOBONamespace>GAZ</oboInOwl:hasOBONamespace>
        <oboInOwl:id>GAZ:00144828</oboInOwl:id>
        <rdfs:label>Gissar Range</rdfs:label>
    </owl:NamedIndividual>
    


    <!-- http://purl.obolibrary.org/obo/GAZ_00144830 -->

    <owl:NamedIndividual rdf:about="http://purl.obolibrary.org/obo/GAZ_00144830">
        <obo:RO_0001025 rdf:resource="http://purl.obolibrary.org/obo/GAZ_00004988"/>
        <obo:IAO_0000115>A mountain range that rises to the south of the Zeravshan River. The range extends over 370 km in the east-west direction along the south of Sughd Province in Tajikistan, reaching the highest point of 5,489 m (Chimtarga peak) in its central part. South-west of Penjikent the range crosses from Tajikistan into Uzbekistan, where it continues at decreasing elevations (1,500-2,000 m) along the internal border between Samarkand and Surkhandarya provinces, until it blends into the desert south-west of Samarkand.</obo:IAO_0000115>
        <oboInOwl:hasOBONamespace>GAZ</oboInOwl:hasOBONamespace>
        <oboInOwl:id>GAZ:00144830</oboInOwl:id>
        <rdfs:label>Zeravshan Range</rdfs:label>
    </owl:NamedIndividual>
    


    <!-- http://purl.obolibrary.org/obo/GAZ_00148842 -->

    <owl:NamedIndividual rdf:about="http://purl.obolibrary.org/obo/GAZ_00148842">
        <obo:RO_0001025 rdf:resource="http://purl.obolibrary.org/obo/GAZ_00006882"/>
        <obo:IAO_0000115>A river in Afghanistan, about 400 km in length. It rises in the Hazarajat country north-west of Ghazni, and flows south-west falls into the Helmund 30 km below Girishk.</obo:IAO_0000115>
        <oboInOwl:hasOBONamespace>GAZ</oboInOwl:hasOBONamespace>
        <oboInOwl:id>GAZ:00148842</oboInOwl:id>
        <rdfs:label>Arghandab River</rdfs:label>
    </owl:NamedIndividual>
    


    <!-- http://purl.obolibrary.org/obo/GAZ_00148843 -->

    <owl:NamedIndividual rdf:about="http://purl.obolibrary.org/obo/GAZ_00148843">
        <obo:RO_0001025 rdf:resource="http://purl.obolibrary.org/obo/GAZ_00010642"/>
        <obo:RO_0001025 rdf:resource="http://purl.obolibrary.org/obo/GAZ_00148842"/>
        <obo:IAO_0000115>A dam on the Arghandab River 34 km north of Kandahar City.</obo:IAO_0000115>
        <oboInOwl:hasOBONamespace>GAZ</oboInOwl:hasOBONamespace>
        <oboInOwl:id>GAZ:00148843</oboInOwl:id>
        <rdfs:label>Dahla Dam</rdfs:label>
    </owl:NamedIndividual>
    


    <!-- http://purl.obolibrary.org/obo/GAZ_00148844 -->

    <owl:NamedIndividual rdf:about="http://purl.obolibrary.org/obo/GAZ_00148844">
        <obo:RO_0001025 rdf:resource="http://purl.obolibrary.org/obo/GAZ_00006882"/>
        <obo:IAO_0000115>The longest river in Afghanistan and the primarily watershed for the endorheic Sistan Basin. The Helmand river stretches for 1,150 km. It rises in the Hindu Kush mountains, about 80 km west of Kabul, passing north of the Unai Pass. It crosses south-west through the desert of Dashti Margo, to the Seistan marshes and the Hamun-i-Helmand lake region around Zabol at the Afghan-Iranian border.</obo:IAO_0000115>
        <oboInOwl:hasOBONamespace>GAZ</oboInOwl:hasOBONamespace>
        <oboInOwl:id>GAZ:00148844</oboInOwl:id>
        <rdfs:label>Helmand River</rdfs:label>
    </owl:NamedIndividual>
    


    <!-- http://purl.obolibrary.org/obo/GAZ_00148845 -->

    <owl:NamedIndividual rdf:about="http://purl.obolibrary.org/obo/GAZ_00148845">
        <obo:RO_0001025 rdf:resource="http://purl.obolibrary.org/obo/GAZ_00010650"/>
        <obo:RO_0001025 rdf:resource="http://purl.obolibrary.org/obo/GAZ_00148844"/>
        <obo:IAO_0000115>A dam and associated reservoir located 55 miles north-west of Kandahar City.</obo:IAO_0000115>
        <oboInOwl:hasOBONamespace>GAZ</oboInOwl:hasOBONamespace>
        <oboInOwl:id>GAZ:00148845</oboInOwl:id>
        <rdfs:label>Kajaki Dam</rdfs:label>
    </owl:NamedIndividual>
    


    <!-- http://purl.obolibrary.org/obo/GAZ_00148846 -->

    <owl:NamedIndividual rdf:about="http://purl.obolibrary.org/obo/GAZ_00148846">
        <obo:RO_0001025 rdf:resource="http://purl.obolibrary.org/obo/GAZ_00010650"/>
        <obo:RO_0001025 rdf:resource="http://purl.obolibrary.org/obo/GAZ_00148844"/>
        <obo:IAO_0000115>A dam on the Helmand River in Helmand Province of Afghanistan.</obo:IAO_0000115>
        <oboInOwl:hasOBONamespace>GAZ</oboInOwl:hasOBONamespace>
        <oboInOwl:id>GAZ:00148846</oboInOwl:id>
        <rdfs:label>Grishk Dam</rdfs:label>
    </owl:NamedIndividual>
    


    <!-- http://purl.obolibrary.org/obo/GAZ_00148865 -->

    <owl:NamedIndividual rdf:about="http://purl.obolibrary.org/obo/GAZ_00148865">
        <obo:IAO_0000115>A dam on the Chambal in Neemuch District of Madhya Pradesh.</obo:IAO_0000115>
        <oboInOwl:hasOBONamespace>GAZ</oboInOwl:hasOBONamespace>
        <oboInOwl:id>GAZ:00148865</oboInOwl:id>
        <rdfs:label>Gandhi Sagar Dam</rdfs:label>
    </owl:NamedIndividual>
    


    <!-- http://purl.obolibrary.org/obo/GAZ_00148866 -->

    <owl:NamedIndividual rdf:about="http://purl.obolibrary.org/obo/GAZ_00148866">
        <obo:IAO_0000115>A dam located 52 km downstream of Gandhi Sagar dam on across the Chambal River near Rawatbhata in Chittorgarh district in Rajasthan. Completed 1970.</obo:IAO_0000115>
        <oboInOwl:hasOBONamespace>GAZ</oboInOwl:hasOBONamespace>
        <oboInOwl:id>GAZ:00148866</oboInOwl:id>
        <rdfs:label>Rana Pratap Sagar Dam</rdfs:label>
    </owl:NamedIndividual>
    


    <!-- http://purl.obolibrary.org/obo/GAZ_00148867 -->

    <owl:NamedIndividual rdf:about="http://purl.obolibrary.org/obo/GAZ_00148867">
        <obo:IAO_0000115>A dam located about 0.8 km upstream of Kota City in Rajasthan.</obo:IAO_0000115>
        <oboInOwl:hasOBONamespace>GAZ</oboInOwl:hasOBONamespace>
        <oboInOwl:id>GAZ:00148867</oboInOwl:id>
        <rdfs:label>Kota Barrage</rdfs:label>
    </owl:NamedIndividual>
    


    <!-- http://purl.obolibrary.org/obo/GAZ_00148868 -->

    <owl:NamedIndividual rdf:about="http://purl.obolibrary.org/obo/GAZ_00148868">
        <obo:IAO_0000115>A dam across the Chambal River. It is situated 24 km south-west of Kota, Rajasthan.</obo:IAO_0000115>
        <oboInOwl:hasOBONamespace>GAZ</oboInOwl:hasOBONamespace>
        <oboInOwl:id>GAZ:00148868</oboInOwl:id>
        <rdfs:label>Jawahar Sagar Dam</rdfs:label>
    </owl:NamedIndividual>
    


    <!-- http://purl.obolibrary.org/obo/GAZ_00148909 -->

    <owl:NamedIndividual rdf:about="http://purl.obolibrary.org/obo/GAZ_00148909">
        <obo:IAO_0000115>An Inter-state Dam project of the Government of Madhya Pradesh and Uttar Pradesh being constructed on Betwa River about 22 km from Lalitpur in Uttar Pradesh, India.</obo:IAO_0000115>
        <oboInOwl:hasOBONamespace>GAZ</oboInOwl:hasOBONamespace>
        <oboInOwl:id>GAZ:00148909</oboInOwl:id>
        <rdfs:label>Rajghat Dam</rdfs:label>
    </owl:NamedIndividual>
    


    <!-- http://purl.obolibrary.org/obo/GAZ_00148911 -->

    <owl:NamedIndividual rdf:about="http://purl.obolibrary.org/obo/GAZ_00148911">
        <obo:IAO_0000115>A reservoir being created by the Rajghat Dam.</obo:IAO_0000115>
        <oboInOwl:hasOBONamespace>GAZ</oboInOwl:hasOBONamespace>
        <oboInOwl:id>GAZ:00148911</oboInOwl:id>
        <rdfs:label>Rajghat Reservoir</rdfs:label>
    </owl:NamedIndividual>
    


    <!-- http://purl.obolibrary.org/obo/GAZ_00148912 -->

    <owl:NamedIndividual rdf:about="http://purl.obolibrary.org/obo/GAZ_00148912">
        <obo:IAO_0000115>A dam in India on the Betwa River. Situated 93 km away from Deogarh, Uttar Pradesh. Constructed 1958.</obo:IAO_0000115>
        <oboInOwl:hasOBONamespace>GAZ</oboInOwl:hasOBONamespace>
        <oboInOwl:id>GAZ:00148912</oboInOwl:id>
        <rdfs:label>Matatila Dam</rdfs:label>
    </owl:NamedIndividual>
    


    <!-- http://purl.obolibrary.org/obo/GAZ_00148913 -->

    <owl:NamedIndividual rdf:about="http://purl.obolibrary.org/obo/GAZ_00148913">
        <obo:IAO_0000115>A dam built on the Betwa River near Parichha town, Uttar Pradesh.</obo:IAO_0000115>
        <oboInOwl:hasOBONamespace>GAZ</oboInOwl:hasOBONamespace>
        <oboInOwl:id>GAZ:00148913</oboInOwl:id>
        <rdfs:label>Parichha Dam</rdfs:label>
    </owl:NamedIndividual>
    


    <!-- http://purl.obolibrary.org/obo/GAZ_00148924 -->

    <owl:NamedIndividual rdf:about="http://purl.obolibrary.org/obo/GAZ_00148924">
        <obo:IAO_0000115>A multi-purpose dam situated in Shivpuri district in Madhya Pradesh, India. Impounds the Madikheda Reservoir. Constructed 1978-2008.</obo:IAO_0000115>
        <oboInOwl:hasOBONamespace>GAZ</oboInOwl:hasOBONamespace>
        <oboInOwl:id>GAZ:00148924</oboInOwl:id>
        <rdfs:label>Madikheda Dam</rdfs:label>
    </owl:NamedIndividual>
    


    <!-- http://purl.obolibrary.org/obo/GAZ_00148925 -->

    <owl:NamedIndividual rdf:about="http://purl.obolibrary.org/obo/GAZ_00148925">
        <obo:IAO_0000115>A reservoir created by the Madikheda Dam. Constructed 1978-2008.</obo:IAO_0000115>
        <oboInOwl:hasOBONamespace>GAZ</oboInOwl:hasOBONamespace>
        <oboInOwl:id>GAZ:00148925</oboInOwl:id>
        <rdfs:label>Madikheda Reservoir</rdfs:label>
    </owl:NamedIndividual>
    


    <!-- http://purl.obolibrary.org/obo/GAZ_00149036 -->

    <owl:NamedIndividual rdf:about="http://purl.obolibrary.org/obo/GAZ_00149036">
        <obo:IAO_0000115>A dam located in Yamuna Nagar District, in the State of Haryana, India. It regulates the flow of the Yamuna for irrigation in Uttar Pradesh and Haryana through two canals originating at this place namely Western Yamuna Canal and Eastern Yamuna Canal, as well as the municipal water supply to Delhi. Completed 1873.</obo:IAO_0000115>
        <oboInOwl:hasOBONamespace>GAZ</oboInOwl:hasOBONamespace>
        <oboInOwl:id>GAZ:00149036</oboInOwl:id>
        <rdfs:label>Tajewala Dam</rdfs:label>
    </owl:NamedIndividual>
    


    <!-- http://purl.obolibrary.org/obo/GAZ_00149059 -->

    <owl:NamedIndividual rdf:about="http://purl.obolibrary.org/obo/GAZ_00149059">
        <obo:RO_0001025 rdf:resource="http://purl.obolibrary.org/obo/GAZ_00149060"/>
        <obo:IAO_0000115>A glacier situated in the Pithoragarh District of Uttarakhand State of India The glacier situated on Kumaon Himalayas at an altitude of 3,600 m.</obo:IAO_0000115>
        <oboInOwl:hasOBONamespace>GAZ</oboInOwl:hasOBONamespace>
        <oboInOwl:id>GAZ:00149059</oboInOwl:id>
        <rdfs:label>Namik Glacier</rdfs:label>
    </owl:NamedIndividual>
    


    <!-- http://purl.obolibrary.org/obo/GAZ_00149060 -->

    <owl:NamedIndividual rdf:about="http://purl.obolibrary.org/obo/GAZ_00149060">
        <oboInOwl:hasOBONamespace>GAZ</oboInOwl:hasOBONamespace>
        <oboInOwl:id>GAZ:00149060</oboInOwl:id>
        <rdfs:label>Kumaon Himalayas</rdfs:label>
    </owl:NamedIndividual>
    


    <!-- http://purl.obolibrary.org/obo/GAZ_00149073 -->

    <owl:NamedIndividual rdf:about="http://purl.obolibrary.org/obo/GAZ_00149073">
        <obo:IAO_0000115>A below water construction on Betwa River near Jhansi District, Uttar Pradesh.</obo:IAO_0000115>
        <oboInOwl:hasOBONamespace>GAZ</oboInOwl:hasOBONamespace>
        <oboInOwl:id>GAZ:00149073</oboInOwl:id>
        <rdfs:label>Sukma-Dukma Dam</rdfs:label>
    </owl:NamedIndividual>
    


    <!-- http://purl.obolibrary.org/obo/GAZ_00149226 -->

    <owl:NamedIndividual rdf:about="http://purl.obolibrary.org/obo/GAZ_00149226">
        <obo:RO_0001025 rdf:resource="http://purl.obolibrary.org/obo/GAZ_00248810"/>
        <obo:IAO_0000115>A protected area located in eastern Haryana, India, 150 km from Chandigarh.</obo:IAO_0000115>
        <oboInOwl:hasOBONamespace>GAZ</oboInOwl:hasOBONamespace>
        <oboInOwl:id>GAZ:00149226</oboInOwl:id>
        <rdfs:label>Kalesar National Park</rdfs:label>
    </owl:NamedIndividual>
    


    <!-- http://purl.obolibrary.org/obo/GAZ_00246580 -->

    <owl:NamedIndividual rdf:about="http://purl.obolibrary.org/obo/GAZ_00246580">
        <obo:RO_0001025 rdf:resource="http://purl.obolibrary.org/obo/GAZ_00004988"/>
        <obo:RO_0001025 rdf:resource="http://purl.obolibrary.org/obo/GAZ_00098853"/>
        <obo:IAO_0000115>A high altitude lake. Located some 45 km southeast of Zorkul. It lies in a broad valley between the Big Pamir and Small Pamir ranges, and is fed by snow-melt from both these ranges. It is about 16 km long and up to 2 km wide. The lake drains through an outlet at its eastern end into the Aksu River, which joins the Pamir River in Tadzhikistan.</obo:IAO_0000115>
        <oboInOwl:hasOBONamespace>GAZ</oboInOwl:hasOBONamespace>
        <oboInOwl:id>GAZ:00246580</oboInOwl:id>
        <rdfs:label>Chaqmatin Lake</rdfs:label>
    </owl:NamedIndividual>
    


    <!-- http://purl.obolibrary.org/obo/GAZ_00246582 -->

    <owl:NamedIndividual rdf:about="http://purl.obolibrary.org/obo/GAZ_00246582">
        <obo:RO_0001025 rdf:resource="http://purl.obolibrary.org/obo/GAZ_00076860"/>
        <obo:IAO_0000115>A small, shallow, slightly saline, eutrophic lake in a basin on a large shelf in the foothills of the Hindu Kush. It is fed by a tributary of the Logar River, and has no outlet except when the water level is exceptionally high.</obo:IAO_0000115>
        <oboInOwl:hasOBONamespace>GAZ</oboInOwl:hasOBONamespace>
        <oboInOwl:id>GAZ:00246582</oboInOwl:id>
        <rdfs:label>Kole Hashmat Khan</rdfs:label>
    </owl:NamedIndividual>
    


    <!-- http://purl.obolibrary.org/obo/GAZ_00246583 -->

    <owl:NamedIndividual rdf:about="http://purl.obolibrary.org/obo/GAZ_00246583">
        <obo:RO_0001025 rdf:resource="http://purl.obolibrary.org/obo/GAZ_00010630"/>
        <obo:IAO_0000115>A freshwater lake located near the city of Jalabad.</obo:IAO_0000115>
        <oboInOwl:hasOBONamespace>GAZ</oboInOwl:hasOBONamespace>
        <oboInOwl:id>GAZ:00246583</oboInOwl:id>
        <rdfs:label>Lake Duronta</rdfs:label>
    </owl:NamedIndividual>
    


    <!-- http://purl.obolibrary.org/obo/GAZ_00246584 -->

    <owl:NamedIndividual rdf:about="http://purl.obolibrary.org/obo/GAZ_00246584">
        <obo:RO_0001025 rdf:resource="http://purl.obolibrary.org/obo/GAZ_00010630"/>
        <obo:IAO_0000115>A lake created by a barrage on the Kabul River.</obo:IAO_0000115>
        <oboInOwl:hasOBONamespace>GAZ</oboInOwl:hasOBONamespace>
        <oboInOwl:id>GAZ:00246584</oboInOwl:id>
        <rdfs:label>Lake Sarobi</rdfs:label>
    </owl:NamedIndividual>
    


    <!-- http://purl.obolibrary.org/obo/GAZ_00246586 -->

    <owl:NamedIndividual rdf:about="http://purl.obolibrary.org/obo/GAZ_00246586">
        <obo:RO_0001025 rdf:resource="http://purl.obolibrary.org/obo/GAZ_00010652"/>
        <obo:RO_0001025 rdf:resource="http://purl.obolibrary.org/obo/GAZ_00246588"/>
        <obo:IAO_0000115>A high desert plateau, about 40 km from north to south and up to 15 km from east to west, in the Koh-i Baba Range of the Hindu Kush. It is surrounded on all sides by mountains rising to peaks in excess of 4,800 m, and contains a shallow, brackish lake, Ab-i Nawar.</obo:IAO_0000115>
        <oboInOwl:hasOBONamespace>GAZ</oboInOwl:hasOBONamespace>
        <oboInOwl:id>GAZ:00246586</oboInOwl:id>
        <rdfs:label>Dashte Nawar</rdfs:label>
    </owl:NamedIndividual>
    


    <!-- http://purl.obolibrary.org/obo/GAZ_00246587 -->

    <owl:NamedIndividual rdf:about="http://purl.obolibrary.org/obo/GAZ_00246587">
        <obo:RO_0001025 rdf:resource="http://purl.obolibrary.org/obo/GAZ_00246586"/>
        <obo:IAO_0000115>A shallow brackish lake.</obo:IAO_0000115>
        <oboInOwl:hasOBONamespace>GAZ</oboInOwl:hasOBONamespace>
        <oboInOwl:id>GAZ:00246587</oboInOwl:id>
        <rdfs:label>Ab-i Nawar</rdfs:label>
    </owl:NamedIndividual>
    


    <!-- http://purl.obolibrary.org/obo/GAZ_00246588 -->

    <owl:NamedIndividual rdf:about="http://purl.obolibrary.org/obo/GAZ_00246588">
        <obo:RO_0001025 rdf:resource="http://purl.obolibrary.org/obo/GAZ_00056902"/>
        <obo:IAO_0000115>A mountain range.</obo:IAO_0000115>
        <oboInOwl:hasOBONamespace>GAZ</oboInOwl:hasOBONamespace>
        <oboInOwl:id>GAZ:00246588</oboInOwl:id>
        <rdfs:label>Koh-i Baba Range</rdfs:label>
    </owl:NamedIndividual>
    


    <!-- http://purl.obolibrary.org/obo/GAZ_00246589 -->

    <owl:NamedIndividual rdf:about="http://purl.obolibrary.org/obo/GAZ_00246589">
        <obo:RO_0001025 rdf:resource="http://purl.obolibrary.org/obo/GAZ_00010652"/>
        <obo:IAO_0000115>A large alkaline lake in the southern foothills of the Hindu Kush. It lies on a gently rolling plateau in the southern foothills of the Koh-i Baba and Koh-i Paghman ranges.</obo:IAO_0000115>
        <oboInOwl:hasOBONamespace>GAZ</oboInOwl:hasOBONamespace>
        <oboInOwl:id>GAZ:00246589</oboInOwl:id>
        <rdfs:label>Ab-i Istada</rdfs:label>
    </owl:NamedIndividual>
    


    <!-- http://purl.obolibrary.org/obo/GAZ_00246590 -->

    <owl:NamedIndividual rdf:about="http://purl.obolibrary.org/obo/GAZ_00246590">
        <obo:RO_0001025 rdf:resource="http://purl.obolibrary.org/obo/GAZ_00056902"/>
        <obo:IAO_0000115>A mountain range.</obo:IAO_0000115>
        <oboInOwl:hasOBONamespace>GAZ</oboInOwl:hasOBONamespace>
        <oboInOwl:id>GAZ:00246590</oboInOwl:id>
        <rdfs:label>Koh-i Paghman Range</rdfs:label>
    </owl:NamedIndividual>
    


    <!-- http://purl.obolibrary.org/obo/GAZ_00247596 -->

    <owl:NamedIndividual rdf:about="http://purl.obolibrary.org/obo/GAZ_00247596">
        <obo:IAO_0000115>A large, deep, freshwater lake and associated marshes in the mountains southwest of Lasa.</obo:IAO_0000115>
        <oboInOwl:hasOBONamespace>GAZ</oboInOwl:hasOBONamespace>
        <oboInOwl:id>GAZ:00247596</oboInOwl:id>
        <rdfs:label>Yangcaoyong Cuo</rdfs:label>
    </owl:NamedIndividual>
    


    <!-- http://purl.obolibrary.org/obo/GAZ_00247597 -->

    <owl:NamedIndividual rdf:about="http://purl.obolibrary.org/obo/GAZ_00247597">
        <obo:IAO_0000115>A large freshwater lake and associated marshes on the north slope of the main Himalayan range. Located 135 km southwest of Lasa, Xizang Zizhiqu.</obo:IAO_0000115>
        <oboInOwl:hasOBONamespace>GAZ</oboInOwl:hasOBONamespace>
        <oboInOwl:id>GAZ:00247597</oboInOwl:id>
        <rdfs:label>Pumuoyong Cuo</rdfs:label>
    </owl:NamedIndividual>
    


    <!-- http://purl.obolibrary.org/obo/GAZ_00247598 -->

    <owl:NamedIndividual rdf:about="http://purl.obolibrary.org/obo/GAZ_00247598">
        <obo:IAO_0000115>A large, brackish or saline lake in an inland drainage basin on the north slope of the main Himalayan range. The lake is fed by snowmelt from the Xixabangma Feng Mountains to the south (peaks to 8,012m). Located south of the Yarlung Zangbo Jiang (Brahmaputra River), 540 km west of Lasa.</obo:IAO_0000115>
        <oboInOwl:hasOBONamespace>GAZ</oboInOwl:hasOBONamespace>
        <oboInOwl:id>GAZ:00247598</oboInOwl:id>
        <rdfs:label>Paiku Co</rdfs:label>
    </owl:NamedIndividual>
    


    <!-- http://purl.obolibrary.org/obo/GAZ_00248637 -->

    <owl:NamedIndividual rdf:about="http://purl.obolibrary.org/obo/GAZ_00248637">
        <obo:RO_0001025 rdf:resource="http://purl.obolibrary.org/obo/GAZ_00021708"/>
        <obo:IAO_0000115>A populated place. A city in eastern Afghanistan. Located at the junction of the Kabul and Kunar rivers near the Laghman valley, Jalalabad is the capital of Nangarhar province.</obo:IAO_0000115>
        <oboInOwl:hasOBONamespace>GAZ</oboInOwl:hasOBONamespace>
        <oboInOwl:id>GAZ:00248637</oboInOwl:id>
        <rdfs:label>Jalalabad</rdfs:label>
    </owl:NamedIndividual>
    


    <!-- http://purl.obolibrary.org/obo/GAZ_00248641 -->

    <owl:NamedIndividual rdf:about="http://purl.obolibrary.org/obo/GAZ_00248641">
        <obo:RO_0001025 rdf:resource="http://purl.obolibrary.org/obo/GAZ_00010643"/>
        <obo:IAO_0000115>A valley in north-central Afghanistan, 150 km north of Kabul, near the Hindu Kush mountain range. Located in the Panjshir Province it is divided by the Panjshir River.</obo:IAO_0000115>
        <oboInOwl:hasOBONamespace>GAZ</oboInOwl:hasOBONamespace>
        <oboInOwl:id>GAZ:00248641</oboInOwl:id>
        <rdfs:label>Panjshir Valley</rdfs:label>
    </owl:NamedIndividual>
    


    <!-- http://purl.obolibrary.org/obo/GAZ_00248643 -->

    <owl:NamedIndividual rdf:about="http://purl.obolibrary.org/obo/GAZ_00248643">
        <rdf:type rdf:resource="http://purl.obolibrary.org/obo/ENVO_00000856"/>
        <obo:RO_0001025 rdf:resource="http://purl.obolibrary.org/obo/GAZ_00021697"/>
        <obo:IAO_0000115>A populated place. A town in Afghanistan, the capital of Laghman Province and center of Mihtarlam District.</obo:IAO_0000115>
        <oboInOwl:hasOBONamespace>GAZ</oboInOwl:hasOBONamespace>
        <oboInOwl:id>GAZ:00248643</oboInOwl:id>
        <rdfs:label>Mihtarlam</rdfs:label>
    </owl:NamedIndividual>
    


    <!-- http://purl.obolibrary.org/obo/GAZ_00248709 -->

    <owl:NamedIndividual rdf:about="http://purl.obolibrary.org/obo/GAZ_00248709">
        <obo:IAO_0000115>A mountain range in the Indian state of Jammu and Kashmir that separates Zanskar from Ladakh.</obo:IAO_0000115>
        <oboInOwl:hasOBONamespace>GAZ</oboInOwl:hasOBONamespace>
        <oboInOwl:id>GAZ:00248709</oboInOwl:id>
        <rdfs:label>Zanskar Range</rdfs:label>
    </owl:NamedIndividual>
    


    <!-- http://purl.obolibrary.org/obo/GAZ_00248721 -->

    <owl:NamedIndividual rdf:about="http://purl.obolibrary.org/obo/GAZ_00248721">
        <obo:IAO_0000115>A river located in Bannu District, North-West Frontier Province, Pakistan.</obo:IAO_0000115>
        <oboInOwl:hasOBONamespace>GAZ</oboInOwl:hasOBONamespace>
        <oboInOwl:id>GAZ:00248721</oboInOwl:id>
        <rdfs:label>Gambila River</rdfs:label>
    </owl:NamedIndividual>
    


    <!-- http://purl.obolibrary.org/obo/GAZ_00248743 -->

    <owl:NamedIndividual rdf:about="http://purl.obolibrary.org/obo/GAZ_00248743">
        <obo:RO_0001025 rdf:resource="http://purl.obolibrary.org/obo/GAZ_00006882"/>
        <obo:IAO_0000115>A river is located in Afghanistan.</obo:IAO_0000115>
        <oboInOwl:hasOBONamespace>GAZ</oboInOwl:hasOBONamespace>
        <oboInOwl:id>GAZ:00248743</oboInOwl:id>
        <rdfs:label>Peche River</rdfs:label>
    </owl:NamedIndividual>
    


    <!-- http://purl.obolibrary.org/obo/GAZ_00248745 -->

    <owl:NamedIndividual rdf:about="http://purl.obolibrary.org/obo/GAZ_00248745">
        <obo:RO_0001025 rdf:resource="http://purl.obolibrary.org/obo/GAZ_00057376"/>
        <obo:IAO_0000115>A glacier in the Great Himalaya subrange of Himalayas. It starts north of an unnamed 6,326 m high peak and flows northeastward, north of Laila Peak (Rupal Valley) and south of Nanga Parbat&apos;s many peaks. The meltwater from the glacier forms Rupal River.</obo:IAO_0000115>
        <oboInOwl:hasOBONamespace>GAZ</oboInOwl:hasOBONamespace>
        <oboInOwl:id>GAZ:00248745</oboInOwl:id>
        <rdfs:label>Rupal Glacier</rdfs:label>
    </owl:NamedIndividual>
    


    <!-- http://purl.obolibrary.org/obo/GAZ_00248809 -->

    <owl:NamedIndividual rdf:about="http://purl.obolibrary.org/obo/GAZ_00248809">
        <obo:RO_0001025 rdf:resource="http://purl.obolibrary.org/obo/GAZ_00248810"/>
        <obo:IAO_0000115>A wetland in the Uttarakhand-Himachal Pradesh border region in Doon Valley, (Dehradun District), northern India, situated at the confluence of the Yamuna Canal and the Assan River and about 11 km from Dak Pathar, and 28 km southwest of Dehradun.</obo:IAO_0000115>
        <oboInOwl:hasOBONamespace>GAZ</oboInOwl:hasOBONamespace>
        <oboInOwl:id>GAZ:00248809</oboInOwl:id>
        <rdfs:label>Assan Barrage</rdfs:label>
    </owl:NamedIndividual>
    


    <!-- http://purl.obolibrary.org/obo/GAZ_00248810 -->

    <owl:NamedIndividual rdf:about="http://purl.obolibrary.org/obo/GAZ_00248810">
        <obo:RO_0001025 rdf:resource="http://purl.obolibrary.org/obo/GAZ_00058368"/>
        <obo:IAO_0000115>A valley located in Sivalik Hills in Uttarakhand, India, home to the capital of Indian state of Uttarakhand, Dehradun.</obo:IAO_0000115>
        <oboInOwl:hasOBONamespace>GAZ</oboInOwl:hasOBONamespace>
        <oboInOwl:id>GAZ:00248810</oboInOwl:id>
        <rdfs:label>Doon Valley</rdfs:label>
    </owl:NamedIndividual>
    


    <!-- http://purl.obolibrary.org/obo/GAZ_00248849 -->

    <owl:NamedIndividual rdf:about="http://purl.obolibrary.org/obo/GAZ_00248849">
        <obo:IAO_0000115>A river flowing in Bhind District of Madhya Pradesh in central India.</obo:IAO_0000115>
        <oboInOwl:hasOBONamespace>GAZ</oboInOwl:hasOBONamespace>
        <oboInOwl:id>GAZ:00248849</oboInOwl:id>
        <rdfs:label>Pahuj River</rdfs:label>
    </owl:NamedIndividual>
    


    <!-- http://purl.obolibrary.org/obo/GAZ_00248855 -->

    <owl:NamedIndividual rdf:about="http://purl.obolibrary.org/obo/GAZ_00248855">
        <rdf:type rdf:resource="http://purl.obolibrary.org/obo/ENVO_00000074"/>
        <obo:IAO_0000115>A barrage.</obo:IAO_0000115>
        <oboInOwl:hasOBONamespace>GAZ</oboInOwl:hasOBONamespace>
        <oboInOwl:id>GAZ:00248855</oboInOwl:id>
        <rdfs:label>Okhla Barrage</rdfs:label>
    </owl:NamedIndividual>
    


    <!-- http://purl.obolibrary.org/obo/GAZ_00250888 -->

    <owl:NamedIndividual rdf:about="http://purl.obolibrary.org/obo/GAZ_00250888">
        <obo:IAO_0000115>A fresh/brackish lake. Located in the Sistan Basin, northwest, west and southwest of Zabol, Sistan/Baluchistan. A Ramsar Site.</obo:IAO_0000115>
        <oboInOwl:hasOBONamespace>GAZ</oboInOwl:hasOBONamespace>
        <oboInOwl:id>GAZ:00250888</oboInOwl:id>
        <rdfs:label>Hamoun-i Sabari</rdfs:label>
    </owl:NamedIndividual>
    


    <!-- http://purl.obolibrary.org/obo/GAZ_00250889 -->

    <owl:NamedIndividual rdf:about="http://purl.obolibrary.org/obo/GAZ_00250889">
        <obo:IAO_0000115>A fresh/brackish lake. Located in the Sistan Basin, northwest, west and southwest of Zabol, Sistan/Baluchistan. A Ramsar Site.</obo:IAO_0000115>
        <oboInOwl:hasOBONamespace>GAZ</oboInOwl:hasOBONamespace>
        <oboInOwl:id>GAZ:00250889</oboInOwl:id>
        <rdfs:label>Hamoun-i Hirmand</rdfs:label>
    </owl:NamedIndividual>
    


    <!-- http://purl.obolibrary.org/obo/GAZ_00250897 -->

    <owl:NamedIndividual rdf:about="http://purl.obolibrary.org/obo/GAZ_00250897">
        <obo:IAO_0000115>A freshwater lake. A Ramsar Site.</obo:IAO_0000115>
        <oboInOwl:hasOBONamespace>GAZ</oboInOwl:hasOBONamespace>
        <oboInOwl:id>GAZ:00250897</oboInOwl:id>
        <rdfs:label>Hamoun-i Puzak</rdfs:label>
    </owl:NamedIndividual>
    


    <!-- http://purl.obolibrary.org/obo/GAZ_00250898 -->

    <owl:NamedIndividual rdf:about="http://purl.obolibrary.org/obo/GAZ_00250898">
        <obo:IAO_0000115>A wteland. It links Hamoon-e-Puzak and Hamoon Saberi. In the medium- and high-water periods.</obo:IAO_0000115>
        <oboInOwl:hasOBONamespace>GAZ</oboInOwl:hasOBONamespace>
        <oboInOwl:id>GAZ:00250898</oboInOwl:id>
        <rdfs:label>Baringak</rdfs:label>
    </owl:NamedIndividual>
    


    <!-- http://purl.obolibrary.org/obo/GAZ_00250899 -->

    <owl:NamedIndividual rdf:about="http://purl.obolibrary.org/obo/GAZ_00250899">
        <obo:IAO_0000115>A wetland. Its large eastern neighbour is Hamoon-e-Puzak, separated by a thin peninsula of higher ground on which a series of villages is located.</obo:IAO_0000115>
        <oboInOwl:hasOBONamespace>GAZ</oboInOwl:hasOBONamespace>
        <oboInOwl:id>GAZ:00250899</oboInOwl:id>
        <rdfs:label>Chonge Sorkh</rdfs:label>
    </owl:NamedIndividual>
    


    <!-- http://purl.obolibrary.org/obo/GAZ_00250903 -->

    <owl:NamedIndividual rdf:about="http://purl.obolibrary.org/obo/GAZ_00250903">
        <obo:RO_0001025 rdf:resource="http://purl.obolibrary.org/obo/GAZ_00021545"/>
        <obo:IAO_0000115>A populated place. A city in western Afghanistan.</obo:IAO_0000115>
        <oboInOwl:hasOBONamespace>GAZ</oboInOwl:hasOBONamespace>
        <oboInOwl:id>GAZ:00250903</oboInOwl:id>
        <rdfs:label>Farah</rdfs:label>
    </owl:NamedIndividual>
    


    <!-- http://purl.obolibrary.org/obo/GAZ_00250904 -->

    <owl:NamedIndividual rdf:about="http://purl.obolibrary.org/obo/GAZ_00250904">
        <obo:IAO_0000115>A reservoir.</obo:IAO_0000115>
        <oboInOwl:hasOBONamespace>GAZ</oboInOwl:hasOBONamespace>
        <oboInOwl:id>GAZ:00250904</oboInOwl:id>
        <rdfs:label>Chah Nimeh Reservoir</rdfs:label>
    </owl:NamedIndividual>
    


    <!-- http://purl.obolibrary.org/obo/GAZ_00250905 -->

    <owl:NamedIndividual rdf:about="http://purl.obolibrary.org/obo/GAZ_00250905">
        <rdf:type rdf:resource="http://purl.obolibrary.org/obo/ENVO_00000104"/>
        <obo:RO_0001025 rdf:resource="http://purl.obolibrary.org/obo/GAZ_00250904"/>
        <obo:IAO_0000115>A basin of the Chah Nimeh Reservoir.</obo:IAO_0000115>
        <oboInOwl:hasOBONamespace>GAZ</oboInOwl:hasOBONamespace>
        <oboInOwl:id>GAZ:00250905</oboInOwl:id>
        <rdfs:label>Basin I, Chah Nimeh Reservoir</rdfs:label>
    </owl:NamedIndividual>
    


    <!-- http://purl.obolibrary.org/obo/GAZ_00250906 -->

    <owl:NamedIndividual rdf:about="http://purl.obolibrary.org/obo/GAZ_00250906">
        <rdf:type rdf:resource="http://purl.obolibrary.org/obo/ENVO_00000104"/>
        <obo:RO_0001025 rdf:resource="http://purl.obolibrary.org/obo/GAZ_00250904"/>
        <obo:IAO_0000115>A basin of the Chah Nimeh Reservoir.</obo:IAO_0000115>
        <oboInOwl:hasOBONamespace>GAZ</oboInOwl:hasOBONamespace>
        <oboInOwl:id>GAZ:00250906</oboInOwl:id>
        <rdfs:label>Basin II, Chah Nimeh Reservoir</rdfs:label>
    </owl:NamedIndividual>
    


    <!-- http://purl.obolibrary.org/obo/GAZ_00250907 -->

    <owl:NamedIndividual rdf:about="http://purl.obolibrary.org/obo/GAZ_00250907">
        <rdf:type rdf:resource="http://purl.obolibrary.org/obo/ENVO_00000104"/>
        <obo:RO_0001025 rdf:resource="http://purl.obolibrary.org/obo/GAZ_00250904"/>
        <obo:IAO_0000115>A basin of the Chah Nimeh Reservoir.</obo:IAO_0000115>
        <oboInOwl:hasOBONamespace>GAZ</oboInOwl:hasOBONamespace>
        <oboInOwl:id>GAZ:00250907</oboInOwl:id>
        <rdfs:label>Basin III, Chah Nimeh Reservoir</rdfs:label>
    </owl:NamedIndividual>
    


    <!-- http://purl.obolibrary.org/obo/GAZ_00250908 -->

    <owl:NamedIndividual rdf:about="http://purl.obolibrary.org/obo/GAZ_00250908">
        <obo:RO_0001025 rdf:resource="http://purl.obolibrary.org/obo/GAZ_00010626"/>
        <obo:IAO_0000115>A saline lake.</obo:IAO_0000115>
        <oboInOwl:hasOBONamespace>GAZ</oboInOwl:hasOBONamespace>
        <oboInOwl:id>GAZ:00250908</oboInOwl:id>
        <rdfs:label>Lake Gowd-e-Zareh</rdfs:label>
    </owl:NamedIndividual>
    


    <!-- http://purl.obolibrary.org/obo/GAZ_00250943 -->

    <owl:NamedIndividual rdf:about="http://purl.obolibrary.org/obo/GAZ_00250943">
        <obo:RO_0001025 rdf:resource="http://purl.obolibrary.org/obo/GAZ_00058500"/>
        <obo:IAO_0000115>A dam. Constructed 1961-1980.</obo:IAO_0000115>
        <oboInOwl:hasOBONamespace>GAZ</oboInOwl:hasOBONamespace>
        <oboInOwl:id>GAZ:00250943</oboInOwl:id>
        <rdfs:label>Nurek Dam</rdfs:label>
    </owl:NamedIndividual>
    


    <!-- http://purl.obolibrary.org/obo/GAZ_00250947 -->

    <owl:NamedIndividual rdf:about="http://purl.obolibrary.org/obo/GAZ_00250947">
        <obo:IAO_0000115>A dam on the Hariroud River, which forms part of the international boundary between Iran and Turkmenistan. Completed 2004.</obo:IAO_0000115>
        <oboInOwl:hasOBONamespace>GAZ</oboInOwl:hasOBONamespace>
        <oboInOwl:id>GAZ:00250947</oboInOwl:id>
        <rdfs:label>Iran-Turkmenistan Friendship Dam</rdfs:label>
    </owl:NamedIndividual>
    


    <!-- http://purl.obolibrary.org/obo/GAZ_00253065 -->

    <owl:NamedIndividual rdf:about="http://purl.obolibrary.org/obo/GAZ_00253065">
        <obo:IAO_0000115>A dead arm of the Kurram River on the west bank of the river about 20 km northwest of Lakki, in a region of irrigated fields and small villages.</obo:IAO_0000115>
        <oboInOwl:hasOBONamespace>GAZ</oboInOwl:hasOBONamespace>
        <oboInOwl:id>GAZ:00253065</oboInOwl:id>
        <rdfs:label>Malugul Dhand</rdfs:label>
    </owl:NamedIndividual>
    


    <!-- 
    ///////////////////////////////////////////////////////////////////////////////////////
    //
    // Annotations
    //
    ///////////////////////////////////////////////////////////////////////////////////////
     -->

    <rdf:Description rdf:about="http://purl.obolibrary.org/obo/GAZ_00009461">
        <rdfs:label>Province (Afghanistan)</rdfs:label>
        <oboInOwl:hasOBONamespace>GAZ</oboInOwl:hasOBONamespace>
        <oboInOwl:id>GAZ:00009461</oboInOwl:id>
    </rdf:Description>
    <rdf:Description rdf:about="http://purl.obolibrary.org/obo/GAZ_00010626">
        <rdfs:label>Nimruz Province</rdfs:label>
        <obo:IAO_0000115>One of the thirty-four provinces of Afghanistan. It is in the south-west of the country on the borders of Iran and Baluchistan.</obo:IAO_0000115>
        <oboInOwl:hasOBONamespace>GAZ</oboInOwl:hasOBONamespace>
        <oboInOwl:id>GAZ:00010626</oboInOwl:id>
    </rdf:Description>
    <rdf:Description rdf:about="http://purl.obolibrary.org/obo/GAZ_00010627">
        <rdfs:label>Laghman Province</rdfs:label>
        <obo:IAO_0000115>One of the thirty-four provinces of Afghanistan. Located in the eastern portion of Afghanistan, the capital is Mihtarlam.</obo:IAO_0000115>
        <oboInOwl:hasOBONamespace>GAZ</oboInOwl:hasOBONamespace>
        <oboInOwl:id>GAZ:00010627</oboInOwl:id>
    </rdf:Description>
    <rdf:Description rdf:about="http://purl.obolibrary.org/obo/GAZ_00010628">
        <rdfs:label>Konduz Province</rdfs:label>
        <oboInOwl:hasOBONamespace>GAZ</oboInOwl:hasOBONamespace>
        <oboInOwl:id>GAZ:00010628</oboInOwl:id>
        <obo:IAO_0000115>One of the provinces of Afghanistan, centered on the city of Kunduz in Afghanistan.</obo:IAO_0000115>
    </rdf:Description>
    <rdf:Description rdf:about="http://purl.obolibrary.org/obo/GAZ_00010629">
        <obo:IAO_0000115>One of the thirty-four provinces of Afghanistan.</obo:IAO_0000115>
        <rdfs:label>Oruzgan Province</rdfs:label>
        <oboInOwl:id>GAZ:00010629</oboInOwl:id>
        <oboInOwl:hasOBONamespace>GAZ</oboInOwl:hasOBONamespace>
    </rdf:Description>
    <rdf:Description rdf:about="http://purl.obolibrary.org/obo/GAZ_00010630">
        <oboInOwl:id>GAZ:00010630</oboInOwl:id>
        <obo:IAO_0000115>One of the thirty-four provinces of Afghanistan. It lies in the east of the country. Its capital is the city of Jalalabad.</obo:IAO_0000115>
        <oboInOwl:hasOBONamespace>GAZ</oboInOwl:hasOBONamespace>
        <rdfs:label>Nangarhar Province</rdfs:label>
    </rdf:Description>
    <rdf:Description rdf:about="http://purl.obolibrary.org/obo/GAZ_00010631">
        <oboInOwl:id>GAZ:00010631</oboInOwl:id>
        <oboInOwl:hasOBONamespace>GAZ</oboInOwl:hasOBONamespace>
        <obo:IAO_0000115>One of the thirty-four provinces of Afghanistan, formed in 1989 and officially established in 2001 from the northern parts of Laghman Province and Kunar Province.</obo:IAO_0000115>
        <rdfs:label>Nurestan Province</rdfs:label>
    </rdf:Description>
    <rdf:Description rdf:about="http://purl.obolibrary.org/obo/GAZ_00010632">
        <oboInOwl:hasOBONamespace>GAZ</oboInOwl:hasOBONamespace>
        <obo:IAO_0000115>One of the thirty-four provinces of Afghanistan, located in the northeastern part of the country and on the border with Pakistan. Its capital is Asadabad.</obo:IAO_0000115>
        <oboInOwl:id>GAZ:00010632</oboInOwl:id>
        <rdfs:label>Konar Province</rdfs:label>
    </rdf:Description>
    <rdf:Description rdf:about="http://purl.obolibrary.org/obo/GAZ_00010633">
        <oboInOwl:id>GAZ:00010633</oboInOwl:id>
        <oboInOwl:hasOBONamespace>GAZ</oboInOwl:hasOBONamespace>
        <obo:IAO_0000115>One of the 34 provinces of Afghanistan. It is located in the eastern zone, southeast of Kabul, and the geography of the province centers on the large Logar River which enters the province through the west and leaves to the north. Its capital is Pul-i-Alam.</obo:IAO_0000115>
        <rdfs:label>Lowgar Province</rdfs:label>
    </rdf:Description>
    <rdf:Description rdf:about="http://purl.obolibrary.org/obo/GAZ_00010634">
        <oboInOwl:id>GAZ:00010634</oboInOwl:id>
        <oboInOwl:hasOBONamespace>GAZ</oboInOwl:hasOBONamespace>
        <rdfs:label>Khost Province</rdfs:label>
        <obo:IAO_0000115>One of the thirty-four provinces of Afghanistan. It is in the east of the country. Its capital is the town also called Khost.</obo:IAO_0000115>
    </rdf:Description>
    <rdf:Description rdf:about="http://purl.obolibrary.org/obo/GAZ_00010635">
        <oboInOwl:id>GAZ:00010635</oboInOwl:id>
        <rdfs:label>Kabul Province</rdfs:label>
        <obo:IAO_0000115>One of the thirty-four provinces of Afghanistan. The capital of the province is Kabul City, which is also the nation&apos;s capital.</obo:IAO_0000115>
        <oboInOwl:hasOBONamespace>GAZ</oboInOwl:hasOBONamespace>
    </rdf:Description>
    <rdf:Description rdf:about="http://purl.obolibrary.org/obo/GAZ_00010636">
        <oboInOwl:id>GAZ:00010636</oboInOwl:id>
        <oboInOwl:hasOBONamespace>GAZ</oboInOwl:hasOBONamespace>
        <obo:IAO_0000115>One of the thirty-four provinces of Afghanistan. It is in the north of the country. Its capital is the city of Sar-e Pol.</obo:IAO_0000115>
        <rdfs:label>Sar-e Pol Province</rdfs:label>
    </rdf:Description>
    <rdf:Description rdf:about="http://purl.obolibrary.org/obo/GAZ_00010637">
        <obo:IAO_0000115>One of the 34 provinces of Afghanistan. It is in the north-east of the country. Its capital is Mahmud-i-Raqi.</obo:IAO_0000115>
        <oboInOwl:hasOBONamespace>GAZ</oboInOwl:hasOBONamespace>
        <rdfs:label>Kapisa Province</rdfs:label>
        <oboInOwl:id>GAZ:00010637</oboInOwl:id>
    </rdf:Description>
    <rdf:Description rdf:about="http://purl.obolibrary.org/obo/GAZ_00010638">
        <oboInOwl:hasOBONamespace>GAZ</oboInOwl:hasOBONamespace>
        <obo:IAO_0000115>One of the thirty-four provinces of Afghanistan. Established 1964 when Qataghan Province was divided into three provinces: Baghlan, Kunduz and Takhar. It is in the north-east of the country. Its capital is Taloqan.</obo:IAO_0000115>
        <oboInOwl:id>GAZ:00010638</oboInOwl:id>
        <rdfs:label>Takhar Province</rdfs:label>
    </rdf:Description>
    <rdf:Description rdf:about="http://purl.obolibrary.org/obo/GAZ_00010639">
        <oboInOwl:id>GAZ:00010639</oboInOwl:id>
        <rdfs:label>Zabol Province</rdfs:label>
        <obo:IAO_0000115>A province of Afghanistan. Zabul became an independent province from neighbouring Kandahar in 1963, with Qalat being named the provincial capital.</obo:IAO_0000115>
        <oboInOwl:hasOBONamespace>GAZ</oboInOwl:hasOBONamespace>
    </rdf:Description>
    <rdf:Description rdf:about="http://purl.obolibrary.org/obo/GAZ_00010640">
        <rdfs:label>Wardak Province</rdfs:label>
        <oboInOwl:id>GAZ:00010640</oboInOwl:id>
        <obo:IAO_0000115>One of the thirty-four provinces of Afghanistan. It is in the centre of the country. Its capital is Meydan Shahr.</obo:IAO_0000115>
        <oboInOwl:hasOBONamespace>GAZ</oboInOwl:hasOBONamespace>
    </rdf:Description>
    <rdf:Description rdf:about="http://purl.obolibrary.org/obo/GAZ_00010641">
        <oboInOwl:hasOBONamespace>GAZ</oboInOwl:hasOBONamespace>
        <oboInOwl:id>GAZ:00010641</oboInOwl:id>
        <rdfs:label>Jowzjan Province</rdfs:label>
        <obo:IAO_0000115>One of the thirty-four provinces of Afghanistan. It is in the north of the country. Its capital is Sheberghan.</obo:IAO_0000115>
    </rdf:Description>
    <rdf:Description rdf:about="http://purl.obolibrary.org/obo/GAZ_00010642">
        <rdfs:label>Kandahar Province</rdfs:label>
        <oboInOwl:hasOBONamespace>GAZ</oboInOwl:hasOBONamespace>
        <oboInOwl:id>GAZ:00010642</oboInOwl:id>
        <obo:IAO_0000115>One of the largest of the thirty-four provinces of Afghanistan. It is located in southern Afghanistan, between Helmand, Oruzgan and Zabul provinces. Its capital is the city of Kandahar, which is located on the Arghandab River.</obo:IAO_0000115>
    </rdf:Description>
    <rdf:Description rdf:about="http://purl.obolibrary.org/obo/GAZ_00010643">
        <oboInOwl:hasOBONamespace>GAZ</oboInOwl:hasOBONamespace>
        <oboInOwl:id>GAZ:00010643</oboInOwl:id>
        <rdfs:label>Panjshir Province</rdfs:label>
        <obo:IAO_0000115>One of the thirty-four provinces of Afghanistan. Containing the Panjshir Valley, it was established from the Parwan Province in 20004-13.</obo:IAO_0000115>
    </rdf:Description>
    <rdf:Description rdf:about="http://purl.obolibrary.org/obo/GAZ_00010644">
        <oboInOwl:hasOBONamespace>GAZ</oboInOwl:hasOBONamespace>
        <oboInOwl:id>GAZ:00010644</oboInOwl:id>
        <rdfs:label>Parvan Province</rdfs:label>
        <obo:IAO_0000115>A province in northern Afghanistan, directly north of Kabul Province. Its capital is Charikar.</obo:IAO_0000115>
    </rdf:Description>
    <rdf:Description rdf:about="http://purl.obolibrary.org/obo/GAZ_00010645">
        <obo:IAO_0000115>One of the thirty-four provinces of Afghanistan. It is in the south-east of the country. Its capital is Sharan.</obo:IAO_0000115>
        <oboInOwl:hasOBONamespace>GAZ</oboInOwl:hasOBONamespace>
        <oboInOwl:id>GAZ:00010645</oboInOwl:id>
        <rdfs:label>Paktika Province</rdfs:label>
    </rdf:Description>
    <rdf:Description rdf:about="http://purl.obolibrary.org/obo/GAZ_00010646">
        <oboInOwl:id>GAZ:00010646</oboInOwl:id>
        <obo:IAO_0000115>One of the thirty-four provinces of Afghanistan, in the east of the country. Its capital is Gardez.</obo:IAO_0000115>
        <rdfs:label>Paktia Province</rdfs:label>
        <oboInOwl:hasOBONamespace>GAZ</oboInOwl:hasOBONamespace>
    </rdf:Description>
    <rdf:Description rdf:about="http://purl.obolibrary.org/obo/GAZ_00010647">
        <oboInOwl:id>GAZ:00010647</oboInOwl:id>
        <obo:IAO_0000115>One of the thirty-four provinces of Afghanistan.</obo:IAO_0000115>
        <oboInOwl:hasOBONamespace>GAZ</oboInOwl:hasOBONamespace>
        <rdfs:label>Samangan Province</rdfs:label>
    </rdf:Description>
    <rdf:Description rdf:about="http://purl.obolibrary.org/obo/GAZ_00010648">
        <oboInOwl:id>GAZ:00010648</oboInOwl:id>
        <obo:IAO_0000115>One of the thirty-four provinces of Afghanistan. It is in the north of the country.</obo:IAO_0000115>
        <rdfs:label>Faryab Province</rdfs:label>
        <oboInOwl:hasOBONamespace>GAZ</oboInOwl:hasOBONamespace>
    </rdf:Description>
    <rdf:Description rdf:about="http://purl.obolibrary.org/obo/GAZ_00010649">
        <obo:IAO_0000115>One of the thirty-four provinces of Afghanistan. It is located in central Afghanistan, towards the north-west.</obo:IAO_0000115>
        <oboInOwl:id>GAZ:00010649</oboInOwl:id>
        <rdfs:label>Ghor Province</rdfs:label>
        <oboInOwl:hasOBONamespace>GAZ</oboInOwl:hasOBONamespace>
    </rdf:Description>
    <rdf:Description rdf:about="http://purl.obolibrary.org/obo/GAZ_00010650">
        <oboInOwl:id>GAZ:00010650</oboInOwl:id>
        <oboInOwl:hasOBONamespace>GAZ</oboInOwl:hasOBONamespace>
        <obo:IAO_0000115>One of the 34 provinces of Afghanistan. It is in the south-west of the country.</obo:IAO_0000115>
        <rdfs:label>Helmand Province</rdfs:label>
    </rdf:Description>
    <rdf:Description rdf:about="http://purl.obolibrary.org/obo/GAZ_00010651">
        <oboInOwl:id>GAZ:00010651</oboInOwl:id>
        <oboInOwl:hasOBONamespace>GAZ</oboInOwl:hasOBONamespace>
        <rdfs:label>Badakhshan Province</rdfs:label>
        <obo:IAO_0000115>One of the 34 provinces of Afghanistan, consisting of 29 districts. It is located in the north-east of the country, between the Hindu Kush and the Amu Darya. Badakshan is primarily bordered by Tajikistan to the north and east. A slim sliver of the province, called the Wakhan Corridor, also extends above northern Pakistan&apos;s Chitral and the disputed Northern Areas of Jammu and Kashmir to a border with China.</obo:IAO_0000115>
    </rdf:Description>
    <rdf:Description rdf:about="http://purl.obolibrary.org/obo/GAZ_00010652">
        <rdfs:label>Ghazni Province</rdfs:label>
        <oboInOwl:id>GAZ:00010652</oboInOwl:id>
        <oboInOwl:hasOBONamespace>GAZ</oboInOwl:hasOBONamespace>
        <obo:IAO_0000115>One of the thirty-four provinces of Afghanistan.</obo:IAO_0000115>
    </rdf:Description>
    <rdf:Description rdf:about="http://purl.obolibrary.org/obo/GAZ_00010653">
        <oboInOwl:id>GAZ:00010653</oboInOwl:id>
        <obo:IAO_0000115>One the 34 Provinces of Afghanistan; together with Badghis, Farah, and Ghor provinces, it makes up the north-western region of the country.</obo:IAO_0000115>
        <oboInOwl:hasOBONamespace>GAZ</oboInOwl:hasOBONamespace>
        <rdfs:label>Herat Province</rdfs:label>
    </rdf:Description>
    <rdf:Description rdf:about="http://purl.obolibrary.org/obo/GAZ_00010654">
        <oboInOwl:id>GAZ:00010654</oboInOwl:id>
        <obo:IAO_0000115>One of the thirty-four provinces of Afghanistan. It is in the north of the country.</obo:IAO_0000115>
        <oboInOwl:hasOBONamespace>GAZ</oboInOwl:hasOBONamespace>
        <rdfs:label>Balkh Province</rdfs:label>
    </rdf:Description>
    <rdf:Description rdf:about="http://purl.obolibrary.org/obo/GAZ_00010655">
        <oboInOwl:hasOBONamespace>GAZ</oboInOwl:hasOBONamespace>
        <oboInOwl:id>GAZ:00010655</oboInOwl:id>
        <rdfs:label>Farah Province</rdfs:label>
        <obo:IAO_0000115>One of the thirty-four provinces of Afghanistan. It is in the west of the country. The province is bounded on the north by Herat, on the northeast by Ghor, the southeast by Helmand, the south by Nimroz, and on the west by Iran.</obo:IAO_0000115>
    </rdf:Description>
    <rdf:Description rdf:about="http://purl.obolibrary.org/obo/GAZ_00010656">
        <oboInOwl:hasOBONamespace>GAZ</oboInOwl:hasOBONamespace>
        <obo:IAO_0000115>One of the thirty-four provinces of Afghanistan. Established 2004-03-28. The region had previously been an isolated district of Uruzgan province.</obo:IAO_0000115>
        <rdfs:label>Daykundi Province</rdfs:label>
        <oboInOwl:id>GAZ:00010656</oboInOwl:id>
    </rdf:Description>
    <rdf:Description rdf:about="http://purl.obolibrary.org/obo/GAZ_00010657">
        <rdfs:label>Bamyan Province</rdfs:label>
        <obo:IAO_0000115>One of the thirty-four provinces of Afghanistan.</obo:IAO_0000115>
        <oboInOwl:hasOBONamespace>GAZ</oboInOwl:hasOBONamespace>
        <oboInOwl:id>GAZ:00010657</oboInOwl:id>
    </rdf:Description>
    <rdf:Description rdf:about="http://purl.obolibrary.org/obo/GAZ_00010658">
        <rdfs:label>Badghis Province</rdfs:label>
        <obo:IAO_0000115>One of the thirty-four provinces of Afghanistan. It is located in northwestern Afghanistan, between the Murghab and Hari rivers, extending as far northward as the edge of the desert of Sarakhs. The province was carved out of portions of Herat and Meymaneh provinces in 1964.</obo:IAO_0000115>
        <oboInOwl:id>GAZ:00010658</oboInOwl:id>
        <oboInOwl:hasOBONamespace>GAZ</oboInOwl:hasOBONamespace>
    </rdf:Description>
    <rdf:Description rdf:about="http://purl.obolibrary.org/obo/GAZ_00010659">
        <oboInOwl:id>GAZ:00010659</oboInOwl:id>
        <rdfs:label>Baghlan Province</rdfs:label>
        <obo:IAO_0000115>One of the thirty-four provinces of Afghanistan. It is in the north of the country.</obo:IAO_0000115>
        <oboInOwl:hasOBONamespace>GAZ</oboInOwl:hasOBONamespace>
    </rdf:Description>
</rdf:RDF>



<!-- Generated by the OWL API (version 4.5.6) https://github.com/owlcs/owlapi -->

