<?xml version="1.0"?>
<rdf:RDF xmlns="http://purl.obolibrary.org/obo/gaz/subsets/countries/Costa_Rica.owl#"
     xml:base="http://purl.obolibrary.org/obo/gaz/subsets/countries/Costa_Rica.owl"
     xmlns:obo="http://purl.obolibrary.org/obo/"
     xmlns:owl="http://www.w3.org/2002/07/owl#"
     xmlns:rdf="http://www.w3.org/1999/02/22-rdf-syntax-ns#"
     xmlns:xml="http://www.w3.org/XML/1998/namespace"
     xmlns:xsd="http://www.w3.org/2001/XMLSchema#"
     xmlns:rdfs="http://www.w3.org/2000/01/rdf-schema#"
     xmlns:oboInOwl="http://www.geneontology.org/formats/oboInOwl#">
    <owl:Ontology rdf:about="http://purl.obolibrary.org/obo/gaz/subsets/countries/Costa_Rica.owl">
        <owl:imports rdf:resource="http://purl.obolibrary.org/obo/gaz/imports/envo_import.owl"/>
        <owl:imports rdf:resource="http://purl.obolibrary.org/obo/gaz/imports/ro_import.owl"/>
    </owl:Ontology>
    


    <!-- 
    ///////////////////////////////////////////////////////////////////////////////////////
    //
    // Annotation properties
    //
    ///////////////////////////////////////////////////////////////////////////////////////
     -->

    


    <!-- http://purl.obolibrary.org/obo/IAO_0000115 -->

    <owl:AnnotationProperty rdf:about="http://purl.obolibrary.org/obo/IAO_0000115"/>
    


    <!-- http://www.geneontology.org/formats/oboInOwl#hasOBONamespace -->

    <owl:AnnotationProperty rdf:about="http://www.geneontology.org/formats/oboInOwl#hasOBONamespace"/>
    


    <!-- http://www.geneontology.org/formats/oboInOwl#id -->

    <owl:AnnotationProperty rdf:about="http://www.geneontology.org/formats/oboInOwl#id"/>
    


    <!-- 
    ///////////////////////////////////////////////////////////////////////////////////////
    //
    // Object Properties
    //
    ///////////////////////////////////////////////////////////////////////////////////////
     -->

    


    <!-- http://purl.obolibrary.org/obo/RO_0001025 -->

    <owl:ObjectProperty rdf:about="http://purl.obolibrary.org/obo/RO_0001025"/>
    


    <!-- 
    ///////////////////////////////////////////////////////////////////////////////////////
    //
    // Classes
    //
    ///////////////////////////////////////////////////////////////////////////////////////
     -->

    


    <!-- http://purl.obolibrary.org/obo/ENVO_00000004 -->

    <owl:Class rdf:about="http://purl.obolibrary.org/obo/ENVO_00000004"/>
    


    <!-- http://purl.obolibrary.org/obo/ENVO_00000032 -->

    <owl:Class rdf:about="http://purl.obolibrary.org/obo/ENVO_00000032"/>
    


    <!-- http://purl.obolibrary.org/obo/ENVO_00000106 -->

    <owl:Class rdf:about="http://purl.obolibrary.org/obo/ENVO_00000106"/>
    


    <!-- http://purl.obolibrary.org/obo/ENVO_00000111 -->

    <owl:Class rdf:about="http://purl.obolibrary.org/obo/ENVO_00000111"/>
    


    <!-- http://purl.obolibrary.org/obo/ENVO_00000354 -->

    <owl:Class rdf:about="http://purl.obolibrary.org/obo/ENVO_00000354"/>
    


    <!-- http://purl.obolibrary.org/obo/GAZ_00003204 -->

    <owl:Class rdf:about="http://purl.obolibrary.org/obo/GAZ_00003204"/>
    


    <!-- http://purl.obolibrary.org/obo/GAZ_00003205 -->

    <owl:Class rdf:about="http://purl.obolibrary.org/obo/GAZ_00003205">
        <rdfs:subClassOf rdf:resource="http://purl.obolibrary.org/obo/GAZ_00003204"/>
    </owl:Class>
    


    <!-- http://purl.obolibrary.org/obo/GAZ_00003206 -->

    <owl:Class rdf:about="http://purl.obolibrary.org/obo/GAZ_00003206">
        <rdfs:subClassOf rdf:resource="http://purl.obolibrary.org/obo/GAZ_00003204"/>
    </owl:Class>
    


    <!-- http://purl.obolibrary.org/obo/GAZ_00003207 -->

    <owl:Class rdf:about="http://purl.obolibrary.org/obo/GAZ_00003207">
        <rdfs:subClassOf rdf:resource="http://purl.obolibrary.org/obo/GAZ_00003204"/>
    </owl:Class>
    


    <!-- http://purl.obolibrary.org/obo/GAZ_00003208 -->

    <owl:Class rdf:about="http://purl.obolibrary.org/obo/GAZ_00003208">
        <rdfs:subClassOf rdf:resource="http://purl.obolibrary.org/obo/GAZ_00003204"/>
    </owl:Class>
    


    <!-- http://purl.obolibrary.org/obo/GAZ_00003209 -->

    <owl:Class rdf:about="http://purl.obolibrary.org/obo/GAZ_00003209">
        <rdfs:subClassOf rdf:resource="http://purl.obolibrary.org/obo/GAZ_00003204"/>
    </owl:Class>
    


    <!-- http://purl.obolibrary.org/obo/GAZ_00003210 -->

    <owl:Class rdf:about="http://purl.obolibrary.org/obo/GAZ_00003210">
        <rdfs:subClassOf rdf:resource="http://purl.obolibrary.org/obo/GAZ_00003204"/>
    </owl:Class>
    


    <!-- http://purl.obolibrary.org/obo/GAZ_00003211 -->

    <owl:Class rdf:about="http://purl.obolibrary.org/obo/GAZ_00003211">
        <rdfs:subClassOf rdf:resource="http://purl.obolibrary.org/obo/GAZ_00003204"/>
    </owl:Class>
    


    <!-- http://purl.obolibrary.org/obo/GAZ_00007370 -->

    <owl:Class rdf:about="http://purl.obolibrary.org/obo/GAZ_00007370"/>
    


    <!-- http://purl.obolibrary.org/obo/GAZ_00007745 -->

    <owl:Class rdf:about="http://purl.obolibrary.org/obo/GAZ_00007745">
        <rdfs:subClassOf rdf:resource="http://purl.obolibrary.org/obo/GAZ_00007370"/>
    </owl:Class>
    


    <!-- http://purl.obolibrary.org/obo/GAZ_00007819 -->

    <owl:Class rdf:about="http://purl.obolibrary.org/obo/GAZ_00007819">
        <rdfs:subClassOf rdf:resource="http://purl.obolibrary.org/obo/GAZ_00007370"/>
    </owl:Class>
    


    <!-- http://purl.obolibrary.org/obo/GAZ_00008824 -->

    <owl:Class rdf:about="http://purl.obolibrary.org/obo/GAZ_00008824">
        <rdfs:subClassOf rdf:resource="http://purl.obolibrary.org/obo/GAZ_00007370"/>
    </owl:Class>
    


    <!-- 
    ///////////////////////////////////////////////////////////////////////////////////////
    //
    // Individuals
    //
    ///////////////////////////////////////////////////////////////////////////////////////
     -->

    


    <!-- http://purl.obolibrary.org/obo/GAZ_00002901 -->

    <owl:NamedIndividual rdf:about="http://purl.obolibrary.org/obo/GAZ_00002901">
        <obo:IAO_0000115>A republic in Central America, bordered by Nicaragua to the north, Panama to the east-southeast, the Pacific Ocean to the west and south, and the Caribbean Sea to the east. Costa Rica is composed of seven provinces, which in turn are divided into 81 cantons.</obo:IAO_0000115>
        <oboInOwl:hasOBONamespace>GAZ</oboInOwl:hasOBONamespace>
        <oboInOwl:id>GAZ:00002901</oboInOwl:id>
        <rdfs:label>Costa Rica</rdfs:label>
    </owl:NamedIndividual>
    


    <!-- http://purl.obolibrary.org/obo/GAZ_00002902 -->

    <owl:NamedIndividual rdf:about="http://purl.obolibrary.org/obo/GAZ_00002902">
        <obo:RO_0001025 rdf:resource="http://purl.obolibrary.org/obo/GAZ_00047498"/>
        <obo:IAO_0000115>An island located off the shore of Costa Rica. It constitutes district 11 (one of 13 districts) of Puntarenas Canton of Puntarenas Province. It is located in the Pacific Ocean, 550 km from the Pacific shore of Costa Rica.</obo:IAO_0000115>
        <oboInOwl:hasOBONamespace>GAZ</oboInOwl:hasOBONamespace>
        <oboInOwl:id>GAZ:00002902</oboInOwl:id>
        <rdfs:label>Cocos Island</rdfs:label>
    </owl:NamedIndividual>
    


    <!-- http://purl.obolibrary.org/obo/GAZ_00002903 -->

    <owl:NamedIndividual rdf:about="http://purl.obolibrary.org/obo/GAZ_00002903">
        <obo:RO_0001025 rdf:resource="http://purl.obolibrary.org/obo/GAZ_00002902"/>
        <oboInOwl:hasOBONamespace>GAZ</oboInOwl:hasOBONamespace>
        <oboInOwl:id>GAZ:00002903</oboInOwl:id>
        <rdfs:label>Dirty Rock</rdfs:label>
    </owl:NamedIndividual>
    


    <!-- http://purl.obolibrary.org/obo/GAZ_00003204 -->

    <owl:NamedIndividual rdf:about="http://purl.obolibrary.org/obo/GAZ_00003204">
        <obo:RO_0001025 rdf:resource="http://purl.obolibrary.org/obo/GAZ_00002901"/>
    </owl:NamedIndividual>
    


    <!-- http://purl.obolibrary.org/obo/GAZ_00003205 -->

    <owl:NamedIndividual rdf:about="http://purl.obolibrary.org/obo/GAZ_00003205"/>
    


    <!-- http://purl.obolibrary.org/obo/GAZ_00003206 -->

    <owl:NamedIndividual rdf:about="http://purl.obolibrary.org/obo/GAZ_00003206"/>
    


    <!-- http://purl.obolibrary.org/obo/GAZ_00003207 -->

    <owl:NamedIndividual rdf:about="http://purl.obolibrary.org/obo/GAZ_00003207"/>
    


    <!-- http://purl.obolibrary.org/obo/GAZ_00003208 -->

    <owl:NamedIndividual rdf:about="http://purl.obolibrary.org/obo/GAZ_00003208"/>
    


    <!-- http://purl.obolibrary.org/obo/GAZ_00003209 -->

    <owl:NamedIndividual rdf:about="http://purl.obolibrary.org/obo/GAZ_00003209"/>
    


    <!-- http://purl.obolibrary.org/obo/GAZ_00003210 -->

    <owl:NamedIndividual rdf:about="http://purl.obolibrary.org/obo/GAZ_00003210"/>
    


    <!-- http://purl.obolibrary.org/obo/GAZ_00003211 -->

    <owl:NamedIndividual rdf:about="http://purl.obolibrary.org/obo/GAZ_00003211"/>
    


    <!-- http://purl.obolibrary.org/obo/GAZ_00003212 -->

    <owl:NamedIndividual rdf:about="http://purl.obolibrary.org/obo/GAZ_00003212">
        <obo:RO_0001025 rdf:resource="http://purl.obolibrary.org/obo/GAZ_00003209"/>
        <obo:IAO_0000115>The eighth canton in the province of Puntarenas in Costa Rica. The canton covers an area of 933.91 km2. Its capital city is San Vito. The upland canton shares its eastern border with Panama. The northern limit is high in the Cordillera de Talamanca, and the southwestern boundary runs through the Fila Zapote, one of many small coastal mountain ranges inland from Costa Rica&apos;s Pacific coast.</obo:IAO_0000115>
        <oboInOwl:hasOBONamespace>GAZ</oboInOwl:hasOBONamespace>
        <oboInOwl:id>GAZ:00003212</oboInOwl:id>
        <rdfs:label>Coto Brus Canton</rdfs:label>
    </owl:NamedIndividual>
    


    <!-- http://purl.obolibrary.org/obo/GAZ_00007370 -->

    <owl:NamedIndividual rdf:about="http://purl.obolibrary.org/obo/GAZ_00007370">
        <obo:RO_0001025 rdf:resource="http://purl.obolibrary.org/obo/GAZ_00002901"/>
    </owl:NamedIndividual>
    


    <!-- http://purl.obolibrary.org/obo/GAZ_00007745 -->

    <owl:NamedIndividual rdf:about="http://purl.obolibrary.org/obo/GAZ_00007745">
        <obo:RO_0001025 rdf:resource="http://purl.obolibrary.org/obo/GAZ_00009457"/>
    </owl:NamedIndividual>
    


    <!-- http://purl.obolibrary.org/obo/GAZ_00007746 -->

    <owl:NamedIndividual rdf:about="http://purl.obolibrary.org/obo/GAZ_00007746">
        <obo:RO_0001025 rdf:resource="http://purl.obolibrary.org/obo/GAZ_00007745"/>
        <oboInOwl:hasOBONamespace>GAZ</oboInOwl:hasOBONamespace>
        <oboInOwl:id>GAZ:00007746</oboInOwl:id>
        <rdfs:label>University of San Jose</rdfs:label>
    </owl:NamedIndividual>
    


    <!-- http://purl.obolibrary.org/obo/GAZ_00007819 -->

    <owl:NamedIndividual rdf:about="http://purl.obolibrary.org/obo/GAZ_00007819">
        <obo:RO_0001025 rdf:resource="http://purl.obolibrary.org/obo/GAZ_00068763"/>
    </owl:NamedIndividual>
    


    <!-- http://purl.obolibrary.org/obo/GAZ_00008824 -->

    <owl:NamedIndividual rdf:about="http://purl.obolibrary.org/obo/GAZ_00008824">
        <obo:RO_0001025 rdf:resource="http://purl.obolibrary.org/obo/GAZ_00068714"/>
    </owl:NamedIndividual>
    


    <!-- http://purl.obolibrary.org/obo/GAZ_00009455 -->

    <owl:NamedIndividual rdf:about="http://purl.obolibrary.org/obo/GAZ_00009455">
        <obo:RO_0001025 rdf:resource="http://purl.obolibrary.org/obo/GAZ_00003211"/>
        <obo:IAO_0000115>The fifth canton in the province of Cartago in Costa Rica. The canton covers an area of 1,642.67 km2. The capital city of the canton is also called Turrialba. The Rio Turrialba and Rio Atirro establish major portions of the canton&apos;s western border, and the Rio Chirripo delineates its long southeastern border.</obo:IAO_0000115>
        <oboInOwl:hasOBONamespace>GAZ</oboInOwl:hasOBONamespace>
        <oboInOwl:id>GAZ:00009455</oboInOwl:id>
        <rdfs:label>Turrialba Canton</rdfs:label>
    </owl:NamedIndividual>
    


    <!-- http://purl.obolibrary.org/obo/GAZ_00009456 -->

    <owl:NamedIndividual rdf:about="http://purl.obolibrary.org/obo/GAZ_00009456">
        <obo:RO_0001025 rdf:resource="http://purl.obolibrary.org/obo/GAZ_00003209"/>
        <obo:IAO_0000115>The seventh canton in the province of Puntarenas in Costa Rica. The canton covers an area of 1,753.96 km2. Its capital city is also called Golfito. The canton encompasses the southernmost Pacific coast of Costa Rica, north from Cerro Punta Gorda at the Panama border. It includes land on both sides of the Golfo Dulce and the entire southern portion of the Osa Peninsula.</obo:IAO_0000115>
        <oboInOwl:hasOBONamespace>GAZ</oboInOwl:hasOBONamespace>
        <oboInOwl:id>GAZ:00009456</oboInOwl:id>
        <rdfs:label>Golfito Canton</rdfs:label>
    </owl:NamedIndividual>
    


    <!-- http://purl.obolibrary.org/obo/GAZ_00009457 -->

    <owl:NamedIndividual rdf:about="http://purl.obolibrary.org/obo/GAZ_00009457">
        <obo:RO_0001025 rdf:resource="http://purl.obolibrary.org/obo/GAZ_00003207"/>
        <obo:IAO_0000115>The first canton in the province of San Jose in Costa Rica. The canton covers an area of 44.62 km2. It is contiguous with the national capital city of San Jose. The canton lies on a fertile plain at the southern end of the Central Valley (Meseta Central). The Rio Virilla and Rio Torres form the border on the north, while the Rio Tiribi marks the southern boundary. The canton encompasses San Jose Centro, although the Greater Metropolitan Area reaches far beyond in all directions.</obo:IAO_0000115>
        <oboInOwl:hasOBONamespace>GAZ</oboInOwl:hasOBONamespace>
        <oboInOwl:id>GAZ:00009457</oboInOwl:id>
        <rdfs:label>San Jose Canton</rdfs:label>
    </owl:NamedIndividual>
    


    <!-- http://purl.obolibrary.org/obo/GAZ_00009458 -->

    <owl:NamedIndividual rdf:about="http://purl.obolibrary.org/obo/GAZ_00009458">
        <obo:RO_0001025 rdf:resource="http://purl.obolibrary.org/obo/GAZ_00003208"/>
        <obo:IAO_0000115>The sixth canton in the province of Heredia in Costa Rica. The canton covers an area of 26.96 km2, The capital city of the canton is also called San Isidro. The canton is in the highlands northeast of the provincial capital city of Heredia. The Rio Para Blanca forms its far northeastern border.</obo:IAO_0000115>
        <oboInOwl:hasOBONamespace>GAZ</oboInOwl:hasOBONamespace>
        <oboInOwl:id>GAZ:00009458</oboInOwl:id>
        <rdfs:label>San Isidro Canton</rdfs:label>
    </owl:NamedIndividual>
    


    <!-- http://purl.obolibrary.org/obo/GAZ_00047498 -->

    <owl:NamedIndividual rdf:about="http://purl.obolibrary.org/obo/GAZ_00047498">
        <obo:RO_0001025 rdf:resource="http://purl.obolibrary.org/obo/GAZ_00003209"/>
        <obo:IAO_0000115>The first canton in the province of Puntarenas in Costa Rica. The canton covers an area of 1,842.33 km2. Its capital is the provincial capital city of Puntarenas. The canton includes areas on both sides of the Gulf of Nicoya. From the western coastline, the canton ranges eastward into the Cordillera de Tilaran to include the Monteverde region. The southern portion of the Nicoya Peninsula is also in the canton.</obo:IAO_0000115>
        <oboInOwl:hasOBONamespace>GAZ</oboInOwl:hasOBONamespace>
        <oboInOwl:id>GAZ:00047498</oboInOwl:id>
        <rdfs:label>Puntarenas Canton</rdfs:label>
    </owl:NamedIndividual>
    


    <!-- http://purl.obolibrary.org/obo/GAZ_00047499 -->

    <owl:NamedIndividual rdf:about="http://purl.obolibrary.org/obo/GAZ_00047499">
        <obo:RO_0001025 rdf:resource="http://purl.obolibrary.org/obo/GAZ_00003209"/>
        <obo:IAO_0000115>A bay of the Pacific Ocean, bounded on the north, east, and southeast by southwestern Costa Rica. The bay, which measures approximately 40 km from northeast to southwest, extends from the town of Quepos southeastward for approximately 100 km to San Pedro (Llorona) Point on the Osa Peninsula. At the mouth of the Grande de Terraba (Diquis) River are numerous islands; farther offshore lies Cano Island. Dominical, on Dominical Point, which protrudes into Coronado Bay, is the principal port.</obo:IAO_0000115>
        <oboInOwl:hasOBONamespace>GAZ</oboInOwl:hasOBONamespace>
        <oboInOwl:id>GAZ:00047499</oboInOwl:id>
        <rdfs:label>Bahia de Coronado</rdfs:label>
    </owl:NamedIndividual>
    


    <!-- http://purl.obolibrary.org/obo/GAZ_00047500 -->

    <owl:NamedIndividual rdf:about="http://purl.obolibrary.org/obo/GAZ_00047500">
        <obo:RO_0001025 rdf:resource="http://purl.obolibrary.org/obo/GAZ_00047499"/>
        <obo:RO_0001025 rdf:resource="http://purl.obolibrary.org/obo/GAZ_00068755"/>
        <obo:IAO_0000115>A small island in the Bahia de Coronado (Bay of Coronado) in Costa Rica. It is on the Pacific Ocean side of Costa Rica, east of the Peninsula de Osa.</obo:IAO_0000115>
        <oboInOwl:hasOBONamespace>GAZ</oboInOwl:hasOBONamespace>
        <oboInOwl:id>GAZ:00047500</oboInOwl:id>
        <rdfs:label>Isla del Cano</rdfs:label>
    </owl:NamedIndividual>
    


    <!-- http://purl.obolibrary.org/obo/GAZ_00051984 -->

    <owl:NamedIndividual rdf:about="http://purl.obolibrary.org/obo/GAZ_00051984">
        <rdf:type rdf:resource="http://purl.obolibrary.org/obo/ENVO_00000354"/>
        <obo:RO_0001025 rdf:resource="http://purl.obolibrary.org/obo/GAZ_00003210"/>
        <obo:RO_0001025 rdf:resource="http://purl.obolibrary.org/obo/GAZ_00056231"/>
        <obo:IAO_0000115>A volcanic complex in the Guanacaste Range. The volcano consists of an elongated, arcuate NW-SE-trending ridge that was constructed within the 15 km wide early Pleistocene Guachipelin caldera, whose rim is exposed on the south side. Rincon de la Vieja, has an estimated volume of 130 cu km and contains at least 9 major eruptive centers. Activity has migrated to the SE, where the youngest-looking craters are located. The twin cone of 1916 m high Santa Maria volcano, the highest peak of the Rincon complex, is located at the eastern end of a smaller, 5 km wide caldera and has a 500-m-wide crater. A plinian eruption producing the 0.25 cu km Rio Blanca tephra about 3500 years ago was the last major magmatic eruption from the volcano. All subsequent eruptions, including numerous historical eruptions possibly dating back to the 16th century, have been from the prominent crater containing a 500-m-wide acid lake (known as the Active Crater) located ENE of Von Seebach crater.</obo:IAO_0000115>
        <oboInOwl:hasOBONamespace>GAZ</oboInOwl:hasOBONamespace>
        <oboInOwl:id>GAZ:00051984</oboInOwl:id>
        <rdfs:label>Rincon de la Vieja Volcano</rdfs:label>
    </owl:NamedIndividual>
    


    <!-- http://purl.obolibrary.org/obo/GAZ_00056144 -->

    <owl:NamedIndividual rdf:about="http://purl.obolibrary.org/obo/GAZ_00056144">
        <obo:IAO_0000115>The part of the Cordillera de Talamanca nearer the lower saddle of the Isthmus of Panama.</obo:IAO_0000115>
        <oboInOwl:hasOBONamespace>GAZ</oboInOwl:hasOBONamespace>
        <oboInOwl:id>GAZ:00056144</oboInOwl:id>
        <rdfs:label>Sierra de Veraguas</rdfs:label>
    </owl:NamedIndividual>
    


    <!-- http://purl.obolibrary.org/obo/GAZ_00056145 -->

    <owl:NamedIndividual rdf:about="http://purl.obolibrary.org/obo/GAZ_00056145">
        <obo:IAO_0000115>The E part of the Cordillera de Talamanca.</obo:IAO_0000115>
        <oboInOwl:hasOBONamespace>GAZ</oboInOwl:hasOBONamespace>
        <oboInOwl:id>GAZ:00056145</oboInOwl:id>
        <rdfs:label>Serrania de Tabasara</rdfs:label>
    </owl:NamedIndividual>
    


    <!-- http://purl.obolibrary.org/obo/GAZ_00056217 -->

    <owl:NamedIndividual rdf:about="http://purl.obolibrary.org/obo/GAZ_00056217">
        <obo:RO_0001025 rdf:resource="http://purl.obolibrary.org/obo/GAZ_00068896"/>
        <obo:IAO_0000115>A 670 m high andesitic volcano that towers above the eastern shores of Lake Arenal, which has been enlarged by a hydroelectric project. Arenal lies along a volcanic chain that has migrated to the NW from the late-Pleistocene Los Perdidos lava domes through the Pleistocene-to-Holocene Chato volcano, which contains a 500-m-wide, lake-filled summit crater. The earliest known eruptions of Arenal took place about 7000 years ago, and it was active concurrently with Cerro Chato until the activity of Chato ended about 3500 years ago. Growth of Arenal has been characterized by periodic major explosive eruptions at several-hundred-year intervals and periods of lava effusion that armor the cone. Arenal&apos;s most recent eruptive period began with a major explosive eruption in 1968. Continuous explosive activity accompanied by slow lava effusion and the occasional emission of pyroclastic flows has occurred since then from vents at the summit and on the upper western flank.</obo:IAO_0000115>
        <oboInOwl:hasOBONamespace>GAZ</oboInOwl:hasOBONamespace>
        <oboInOwl:id>GAZ:00056217</oboInOwl:id>
        <rdfs:label>Volcan Arenal</rdfs:label>
    </owl:NamedIndividual>
    


    <!-- http://purl.obolibrary.org/obo/GAZ_00056218 -->

    <owl:NamedIndividual rdf:about="http://purl.obolibrary.org/obo/GAZ_00056218">
        <obo:RO_0001025 rdf:resource="http://purl.obolibrary.org/obo/GAZ_00003205"/>
        <obo:RO_0001025 rdf:resource="http://purl.obolibrary.org/obo/GAZ_00068674"/>
        <obo:IAO_0000115>A reservoir in Costa Rica, formed by enlarging an existing small lake of the same name by the completion of a dam in 1979. It is located near the Arenal Volcano and the Monteverde cloud forest.</obo:IAO_0000115>
        <oboInOwl:hasOBONamespace>GAZ</oboInOwl:hasOBONamespace>
        <oboInOwl:id>GAZ:00056218</oboInOwl:id>
        <rdfs:label>Laguna de Arenal</rdfs:label>
    </owl:NamedIndividual>
    


    <!-- http://purl.obolibrary.org/obo/GAZ_00056220 -->

    <owl:NamedIndividual rdf:about="http://purl.obolibrary.org/obo/GAZ_00056220">
        <obo:RO_0001025 rdf:resource="http://purl.obolibrary.org/obo/GAZ_00068896"/>
        <obo:IAO_0000115>A Pleistocene-to-Holocene stratovolcano.</obo:IAO_0000115>
        <oboInOwl:hasOBONamespace>GAZ</oboInOwl:hasOBONamespace>
        <oboInOwl:id>GAZ:00056220</oboInOwl:id>
        <rdfs:label>Volcan Chato</rdfs:label>
    </owl:NamedIndividual>
    


    <!-- http://purl.obolibrary.org/obo/GAZ_00056221 -->

    <owl:NamedIndividual rdf:about="http://purl.obolibrary.org/obo/GAZ_00056221">
        <obo:RO_0001025 rdf:resource="http://purl.obolibrary.org/obo/GAZ_00003205"/>
        <obo:IAO_0000115>The 10th canton in the province of Alajuela in Costa Rica. The canton encompasses a major portion of the Llanura de San Carlos (San Carlos Plain), a wide expanse on the Caribbean side of the Cordillera Central (Central Mountain Range). San Carlos reaches north to the border of Nicaragua, east to the province of Heredia, west to the province of Guanacaste, and south into the heights of the Cordillera.</obo:IAO_0000115>
        <oboInOwl:hasOBONamespace>GAZ</oboInOwl:hasOBONamespace>
        <oboInOwl:id>GAZ:00056221</oboInOwl:id>
        <rdfs:label>San Carlos Canton</rdfs:label>
    </owl:NamedIndividual>
    


    <!-- http://purl.obolibrary.org/obo/GAZ_00056222 -->

    <owl:NamedIndividual rdf:about="http://purl.obolibrary.org/obo/GAZ_00056222">
        <rdf:type rdf:resource="http://purl.obolibrary.org/obo/ENVO_00000106"/>
        <obo:RO_0001025 rdf:resource="http://purl.obolibrary.org/obo/GAZ_00002901"/>
        <obo:IAO_0000115>A range of mountains in central Costa Rica which continues the Continental Divide east of Cordillera de Tilaran. It has four large volcanoes Poas, Barva, Irazu and Turrialba. The highest peak is Irazu at 3,432 m.</obo:IAO_0000115>
        <oboInOwl:hasOBONamespace>GAZ</oboInOwl:hasOBONamespace>
        <oboInOwl:id>GAZ:00056222</oboInOwl:id>
        <rdfs:label>Cordillera Central</rdfs:label>
    </owl:NamedIndividual>
    


    <!-- http://purl.obolibrary.org/obo/GAZ_00056223 -->

    <owl:NamedIndividual rdf:about="http://purl.obolibrary.org/obo/GAZ_00056223">
        <obo:RO_0001025 rdf:resource="http://purl.obolibrary.org/obo/GAZ_00056222"/>
        <obo:RO_0001025 rdf:resource="http://purl.obolibrary.org/obo/GAZ_00068668"/>
        <obo:RO_0001025 rdf:resource="http://purl.obolibrary.org/obo/GAZ_00068910"/>
        <obo:IAO_0000115>An active stratovolcano that rises to 3432 m immediately east of the capital city of San Jose. The massive volcano covers an area of 500 km2 and is vegetated to within a few hundred meters of its broad flat-topped summit crater complex. At least 10 satellitic cones are located on the southern flank of Irazu. No lava flows have been identified from Irazu since the eruption of the massive Cervantes lava flows from south-flank vents about 14,000 years ago, and all known Holocene eruptions have been explosive. The focus of eruptions at the summit crater complex has migrated to the west towards the historically active crater, which contains a small lake of variable size and color. Although eruptions may have occurred around the time of the Spanish conquest, the first well-documented historical eruption occurred in 1723, and frequent explosive eruptions have occurred since. Ashfall from the last major eruption of Irazu during 1963-65 caused significant disruption to San Jose and surrounding areas.</obo:IAO_0000115>
        <oboInOwl:hasOBONamespace>GAZ</oboInOwl:hasOBONamespace>
        <oboInOwl:id>GAZ:00056223</oboInOwl:id>
        <rdfs:label>Volcan Irazu</rdfs:label>
    </owl:NamedIndividual>
    


    <!-- http://purl.obolibrary.org/obo/GAZ_00056224 -->

    <owl:NamedIndividual rdf:about="http://purl.obolibrary.org/obo/GAZ_00056224">
        <obo:RO_0001025 rdf:resource="http://purl.obolibrary.org/obo/GAZ_00056222"/>
        <obo:RO_0001025 rdf:resource="http://purl.obolibrary.org/obo/GAZ_00068906"/>
        <obo:IAO_0000115>A stratovolcao that is the easternmost of Costa Rica&apos;s Holocene volcanoes, is a large vegetated basaltic-to-dacitic stratovolcano located across a broad saddle NE of Iraze volcano overlooking the city of Cartago. The massive 3340 m high Turrialba is exceeded in height only by Iraze, covers an area of 500 sq km, and is one of Costa Rica&apos;s most voluminous volcanoes. Three well-defined craters occur at the upper SW end of a broad 800 x 2200 m wide summit depression that is breached to the NE. Most activity at Turrialba originated from the summit vent complex, but two pyroclastic cones are located on the SW flank. Five major explosive eruptions have occurred at Turrialba during the past 3500 years. Turrialba has been quiescent since a series of explosive eruptions during the 19th century that were sometimes accompanied by pyroclastic flows. Fumarolic activity continues at the central and SW summit craters.</obo:IAO_0000115>
        <oboInOwl:hasOBONamespace>GAZ</oboInOwl:hasOBONamespace>
        <oboInOwl:id>GAZ:00056224</oboInOwl:id>
        <rdfs:label>Volcan Turrialba</rdfs:label>
    </owl:NamedIndividual>
    


    <!-- http://purl.obolibrary.org/obo/GAZ_00056225 -->

    <owl:NamedIndividual rdf:about="http://purl.obolibrary.org/obo/GAZ_00056225">
        <obo:RO_0001025 rdf:resource="http://purl.obolibrary.org/obo/GAZ_00056222"/>
        <obo:RO_0001025 rdf:resource="http://purl.obolibrary.org/obo/GAZ_00068709"/>
        <obo:IAO_0000115>A complex volcano with multiple summit and flank vents. Its three principal summits visible from the Central Valley give it the common local name of Las Tres Marias. The voluminous andesitic-to-dacitic Tiribi Tuff, exposed in the Central Valley of Costa Rica, was erupted about 322,000 years ago from the Barva summit caldera. Four pyroclastic cones are constructed within the 2 x 3 km caldera at the central and NW part of the summit. The SW peak contains four cones, one of which has a crater lake. Satellitic cones are found on the northern and southern flanks. Lava flows blanket the south side of Barva volcano. The Los Angeles flow, one of the most recent, descends nearly to the city of Heredia. A large plinian eruption occurred at Barva during the early Holocene.</obo:IAO_0000115>
        <oboInOwl:hasOBONamespace>GAZ</oboInOwl:hasOBONamespace>
        <oboInOwl:id>GAZ:00056225</oboInOwl:id>
        <rdfs:label>Volcan Barva</rdfs:label>
    </owl:NamedIndividual>
    


    <!-- http://purl.obolibrary.org/obo/GAZ_00056226 -->

    <owl:NamedIndividual rdf:about="http://purl.obolibrary.org/obo/GAZ_00056226">
        <obo:RO_0001025 rdf:resource="http://purl.obolibrary.org/obo/GAZ_00056222"/>
        <obo:RO_0001025 rdf:resource="http://purl.obolibrary.org/obo/GAZ_00056227"/>
        <obo:IAO_0000115>A stratovolcano that contains three craters along a N-S line. A N-S-trending fissure cutting the 2708 m high complex stratovolcano extends to the lower northern flank, where it has produced the Congo stratovolcano and several lake-filled maars. The southernmost of the two summit crater lakes, Botos, is cold and clear and last erupted about 7500 years ago. The more prominent geothermally heated northern lake, Laguna Caliente, is one of the world&apos;s most acidic natural lakes, with a pH of near zero. It has been the site of frequent phreatic and phreatomagmatic eruptions since the first historical eruption was reported in 1828. Poas eruptions often include geyser-like ejections of crater-lake water.</obo:IAO_0000115>
        <oboInOwl:hasOBONamespace>GAZ</oboInOwl:hasOBONamespace>
        <oboInOwl:id>GAZ:00056226</oboInOwl:id>
        <rdfs:label>Volcan Poas</rdfs:label>
    </owl:NamedIndividual>
    


    <!-- http://purl.obolibrary.org/obo/GAZ_00056227 -->

    <owl:NamedIndividual rdf:about="http://purl.obolibrary.org/obo/GAZ_00056227">
        <obo:RO_0001025 rdf:resource="http://purl.obolibrary.org/obo/GAZ_00002901"/>
        <obo:RO_0001025 rdf:resource="http://purl.obolibrary.org/obo/GAZ_00003205"/>
        <obo:RO_0001025 rdf:resource="http://purl.obolibrary.org/obo/GAZ_00068897"/>
        <obo:IAO_0000115>A national park in Costa Rica that covers an area of approximately 65 km2; the summit is 2,708 m.</obo:IAO_0000115>
        <oboInOwl:hasOBONamespace>GAZ</oboInOwl:hasOBONamespace>
        <oboInOwl:id>GAZ:00056227</oboInOwl:id>
        <rdfs:label>Parque Nacional Volcan Poas</rdfs:label>
    </owl:NamedIndividual>
    


    <!-- http://purl.obolibrary.org/obo/GAZ_00056229 -->

    <owl:NamedIndividual rdf:about="http://purl.obolibrary.org/obo/GAZ_00056229">
        <obo:RO_0001025 rdf:resource="http://purl.obolibrary.org/obo/GAZ_00068895"/>
        <obo:IAO_0000115>A 2028 m high andesitic stratovolcano that is one of five post-caldera cones along a NE-trending line within the broad 15 x 20 km Guayabo (Miravalles) caldera. The caldera was formed during several major explosive eruptions that produced voluminous dacitic-rhyolitic pyroclastic flows between about 1.5 and 0.6 million years ago. Growth of post-caldera volcanoes in the eastern part of the caldera that overtopped much of the eastern and southern caldera rims was interrupted by edifice collapse that produced a major debris avalanche to the SW. Morphologically youthful lava flows cover the western and SW flanks of the post-caldera Miravalles complex, which rises above the town of Guayabo on the flat western caldera floor. The only reported historical eruptive activity was a small steam explosion on the SW flank in 1946. High heat flow remains, and Miravalles is the site of the largest developed geothermal field in Costa Rica.</obo:IAO_0000115>
        <oboInOwl:hasOBONamespace>GAZ</oboInOwl:hasOBONamespace>
        <oboInOwl:id>GAZ:00056229</oboInOwl:id>
        <rdfs:label>Volcan Miravalles</rdfs:label>
    </owl:NamedIndividual>
    


    <!-- http://purl.obolibrary.org/obo/GAZ_00056230 -->

    <owl:NamedIndividual rdf:about="http://purl.obolibrary.org/obo/GAZ_00056230">
        <obo:IAO_0000115>One of a cluster of four eroded and vegetated cones in the Guanacaste Range at the NW corner of Costa Rica. Volcan Orosi itself has a conical shape as viewed from the north or west, but its flanks are heavily eroded. The complex includes Orosi, Orosilito, Volcan Pedregal, and Cacao. The highest peak of the volcanic complex is 1659 m high Volcan Cacao, 5.5 km SE of Orosi. The summit of Cacao is cut by two large horseshoe-shaped calderas breached to the SW and east related to edifice collapse. The age of the latest activity of the Orosi complex is not known. Historical eruptions were reported from Orosi in 1844 and 1849, but even at the time of the first volcanological observations at the end of the 19th century, Orosi was overgrown with large trees, and the eruptions may actually have been from neighboring Rincon de la Vieja volcano. The latest documented volcanic activity at Orosi produced mudflows (perhaps secondary) about 3500 years ago.</obo:IAO_0000115>
        <oboInOwl:hasOBONamespace>GAZ</oboInOwl:hasOBONamespace>
        <oboInOwl:id>GAZ:00056230</oboInOwl:id>
        <rdfs:label>Orosi Volcanic Complex</rdfs:label>
    </owl:NamedIndividual>
    


    <!-- http://purl.obolibrary.org/obo/GAZ_00056231 -->

    <owl:NamedIndividual rdf:about="http://purl.obolibrary.org/obo/GAZ_00056231">
        <obo:RO_0001025 rdf:resource="http://purl.obolibrary.org/obo/GAZ_00068700"/>
        <obo:IAO_0000115>A remote volcanic complex in the Guanacaste Range. The volcano consists of an elongated, arcuate NW-SE-trending ridge that was constructed within the 15 km wide early Pleistocene Guachipelin caldera, whose rim is exposed on the south side. Rincon de la Vieja has an estimated volume of 130 cu km and contains at least 9 major eruptive centers. Activity has migrated to the SE, where the youngest-looking craters are located. The twin cone of 1916 m high Santa Maria volcano, the highest peak of the Rincon complex, is located at the eastern end of a smaller, 5 km wide caldera and has a 500-m-wide crater. A plinian eruption producing the 0.25 cu km Rio Blanca tephra about 3500 years ago was the last major magmatic eruption from the volcano. All subsequent eruptions, including numerous historical eruptions possibly dating back to the 16th century, have been from the prominent crater containing a 500-m-wide acid lake (known as the Active Crater) located ENE of Von Seebach crater.</obo:IAO_0000115>
        <oboInOwl:hasOBONamespace>GAZ</oboInOwl:hasOBONamespace>
        <oboInOwl:id>GAZ:00056231</oboInOwl:id>
        <rdfs:label>Rincon de la Vieja Volcanic Complex</rdfs:label>
    </owl:NamedIndividual>
    


    <!-- http://purl.obolibrary.org/obo/GAZ_00056232 -->

    <owl:NamedIndividual rdf:about="http://purl.obolibrary.org/obo/GAZ_00056232">
        <obo:RO_0001025 rdf:resource="http://purl.obolibrary.org/obo/GAZ_00056230"/>
        <obo:IAO_0000115>A stratovolcano.</obo:IAO_0000115>
        <oboInOwl:hasOBONamespace>GAZ</oboInOwl:hasOBONamespace>
        <oboInOwl:id>GAZ:00056232</oboInOwl:id>
        <rdfs:label>Volcan Cacao</rdfs:label>
    </owl:NamedIndividual>
    


    <!-- http://purl.obolibrary.org/obo/GAZ_00056233 -->

    <owl:NamedIndividual rdf:about="http://purl.obolibrary.org/obo/GAZ_00056233">
        <obo:RO_0001025 rdf:resource="http://purl.obolibrary.org/obo/GAZ_00056230"/>
        <obo:IAO_0000115>A stratovolcano.</obo:IAO_0000115>
        <oboInOwl:hasOBONamespace>GAZ</oboInOwl:hasOBONamespace>
        <oboInOwl:id>GAZ:00056233</oboInOwl:id>
        <rdfs:label>Volcan Pedregal</rdfs:label>
    </owl:NamedIndividual>
    


    <!-- http://purl.obolibrary.org/obo/GAZ_00056234 -->

    <owl:NamedIndividual rdf:about="http://purl.obolibrary.org/obo/GAZ_00056234">
        <obo:RO_0001025 rdf:resource="http://purl.obolibrary.org/obo/GAZ_00056230"/>
        <obo:IAO_0000115>A stratovolcano.</obo:IAO_0000115>
        <oboInOwl:hasOBONamespace>GAZ</oboInOwl:hasOBONamespace>
        <oboInOwl:id>GAZ:00056234</oboInOwl:id>
        <rdfs:label>Volcan Orosi</rdfs:label>
    </owl:NamedIndividual>
    


    <!-- http://purl.obolibrary.org/obo/GAZ_00056235 -->

    <owl:NamedIndividual rdf:about="http://purl.obolibrary.org/obo/GAZ_00056235">
        <obo:RO_0001025 rdf:resource="http://purl.obolibrary.org/obo/GAZ_00056230"/>
        <obo:IAO_0000115>A stratovolcano.</obo:IAO_0000115>
        <oboInOwl:hasOBONamespace>GAZ</oboInOwl:hasOBONamespace>
        <oboInOwl:id>GAZ:00056235</oboInOwl:id>
        <rdfs:label>Volcan Orosilito</rdfs:label>
    </owl:NamedIndividual>
    


    <!-- http://purl.obolibrary.org/obo/GAZ_00056236 -->

    <owl:NamedIndividual rdf:about="http://purl.obolibrary.org/obo/GAZ_00056236">
        <obo:RO_0001025 rdf:resource="http://purl.obolibrary.org/obo/GAZ_00003205"/>
        <obo:RO_0001025 rdf:resource="http://purl.obolibrary.org/obo/GAZ_00264527"/>
        <obo:IAO_0000115>A 225 km2 dominantly andesitic volcanic massif that anchors the SE end of the Guanacaste Range and consists of a cluster of densely forested NNW-SSE-trending volcanic cones. Overlapping lava flows from the principal peak, Tenorio, blanket the NW-to-SW flanks and descend the NE flank. The NW-most of three craters of the central cone is sparsely vegetated and appears to be the most recently active. Volcan Montezuma to the north has twin craters, the northern of which fed a lava flow to the NE. Additional pyroclastic cones are found to the NE and SW of the central complex, and the Bijagua lava domes were constructed on the northern flank. A major debris avalanche covered about 100 km2 below the southern flank of the volcano. Fumarolic activity is present on the NE flank.</obo:IAO_0000115>
        <oboInOwl:hasOBONamespace>GAZ</oboInOwl:hasOBONamespace>
        <oboInOwl:id>GAZ:00056236</oboInOwl:id>
        <rdfs:label>Tenorio Volcanic Massif</rdfs:label>
    </owl:NamedIndividual>
    


    <!-- http://purl.obolibrary.org/obo/GAZ_00056237 -->

    <owl:NamedIndividual rdf:about="http://purl.obolibrary.org/obo/GAZ_00056237">
        <obo:RO_0001025 rdf:resource="http://purl.obolibrary.org/obo/GAZ_00056222"/>
        <obo:IAO_0000115>A volcanic center is the NW-most volcano in the Cordillera Central of Costa Rica. The massive complex covers about 900 km2 and is dominated by two largely Pleistocene stratovolcanoes, Platanar and Porvenir. These volcanoes were constructed within the Pleistocene Chocosuela caldera, which may have formed during a major slope failure. The 2183 m high Cerro Platanar volcano (known locally as Volcan Congo) on the north side of the complex has prehistorical lava flows on its western flanks and is the youngest volcanic center. The highest peak of the complex is 2267 m high Porvenir volcano, whose summit crater lies 3 km south of Platanar. A thin layer of phreatic ash suggested that an eruption from Platanar occurred within the past few thousand years (Stine and Banks, 1991). The Aguas Zarcas group of nine basaltic cinder cones, located on the north flank of the Platanar-Porvenir complex to as low as 160 m altitude, is in part Holocene in age.</obo:IAO_0000115>
        <oboInOwl:hasOBONamespace>GAZ</oboInOwl:hasOBONamespace>
        <oboInOwl:id>GAZ:00056237</oboInOwl:id>
        <rdfs:label>Platanar Volcanic Complex</rdfs:label>
    </owl:NamedIndividual>
    


    <!-- http://purl.obolibrary.org/obo/GAZ_00056238 -->

    <owl:NamedIndividual rdf:about="http://purl.obolibrary.org/obo/GAZ_00056238">
        <obo:RO_0001025 rdf:resource="http://purl.obolibrary.org/obo/GAZ_00056237"/>
        <obo:IAO_0000115>A Pleistocene stratovolcano.</obo:IAO_0000115>
        <oboInOwl:hasOBONamespace>GAZ</oboInOwl:hasOBONamespace>
        <oboInOwl:id>GAZ:00056238</oboInOwl:id>
        <rdfs:label>Platanar Volcano</rdfs:label>
    </owl:NamedIndividual>
    


    <!-- http://purl.obolibrary.org/obo/GAZ_00056239 -->

    <owl:NamedIndividual rdf:about="http://purl.obolibrary.org/obo/GAZ_00056239">
        <obo:RO_0001025 rdf:resource="http://purl.obolibrary.org/obo/GAZ_00056237"/>
        <obo:IAO_0000115>A Pleistocene stratovolcano.</obo:IAO_0000115>
        <oboInOwl:hasOBONamespace>GAZ</oboInOwl:hasOBONamespace>
        <oboInOwl:id>GAZ:00056239</oboInOwl:id>
        <rdfs:label>Porvenir Volcano</rdfs:label>
    </owl:NamedIndividual>
    


    <!-- http://purl.obolibrary.org/obo/GAZ_00056240 -->

    <owl:NamedIndividual rdf:about="http://purl.obolibrary.org/obo/GAZ_00056240">
        <obo:RO_0001025 rdf:resource="http://purl.obolibrary.org/obo/GAZ_00056226"/>
        <obo:IAO_0000115>A very acidic crater lake.</obo:IAO_0000115>
        <oboInOwl:hasOBONamespace>GAZ</oboInOwl:hasOBONamespace>
        <oboInOwl:id>GAZ:00056240</oboInOwl:id>
        <rdfs:label>Laguna Caliente</rdfs:label>
    </owl:NamedIndividual>
    


    <!-- http://purl.obolibrary.org/obo/GAZ_00056241 -->

    <owl:NamedIndividual rdf:about="http://purl.obolibrary.org/obo/GAZ_00056241">
        <obo:RO_0001025 rdf:resource="http://purl.obolibrary.org/obo/GAZ_00090259"/>
        <obo:IAO_0000115>A complex dominantly andesitic stratovolcano in the Talamanca Range near the Costa Rica border. The forested 3474 m high Volcan Baru is the highest peak in Panama, and the summit now bristles with communication towers. A large 6 km wide summit caldera breached widely to the west was formed by a large volcanic landslide, which created a massive debris-avalanche deposit that extends onto the Pacific coastal plain. Post-collapse eruptions have constructed lava domes inside the caldera that have grown to a height exceeding that of the caldera rim.</obo:IAO_0000115>
        <oboInOwl:hasOBONamespace>GAZ</oboInOwl:hasOBONamespace>
        <oboInOwl:id>GAZ:00056241</oboInOwl:id>
        <rdfs:label>Volcan Baru</rdfs:label>
    </owl:NamedIndividual>
    


    <!-- http://purl.obolibrary.org/obo/GAZ_00056243 -->

    <owl:NamedIndividual rdf:about="http://purl.obolibrary.org/obo/GAZ_00056243">
        <obo:RO_0001025 rdf:resource="http://purl.obolibrary.org/obo/GAZ_00056145"/>
        <obo:IAO_0000115>A massive volcanic complex in west-central Panama north of the Azuero Peninsula that was active from the Miocene into the Quaternary. The youngest major feature of La Yeguada is located within a large fault-bounded horst that forms the high point of the volcanic complex east of Laguna La Yeguada. The latest eruptions took place from the northern part of the horst about 220,000 years ago at Cerro Corero lava dome (also known as Cerro de la Charca), north of El Castillo. The youngest feature of the La Yeguada complex is the Media Luna cinder cone, which was erupted through Tertiary ignimbrite deposits at the NW side of the complex. The oldest peat layer within a small lake dammed by a basaltic lava flow originating from the cone was radiocarbon dated at about 300-350 years ago. Warm springs are scattered throughout the complex, and the Chitra-Calobre geothermal field is one of three areas in Panama that have been the object of intensive geothermal exploration.</obo:IAO_0000115>
        <oboInOwl:hasOBONamespace>GAZ</oboInOwl:hasOBONamespace>
        <oboInOwl:id>GAZ:00056243</oboInOwl:id>
        <rdfs:label>La Yeguada Volcano</rdfs:label>
    </owl:NamedIndividual>
    


    <!-- http://purl.obolibrary.org/obo/GAZ_00068645 -->

    <owl:NamedIndividual rdf:about="http://purl.obolibrary.org/obo/GAZ_00068645">
        <obo:RO_0001025 rdf:resource="http://purl.obolibrary.org/obo/GAZ_00003205"/>
        <obo:IAO_0000115>The eighth canton in the province of Alajuela in Costa Rica. The canton covers an area of 73.84 km2. The capital city of the canton is San Pedro. The elongated canton sits among the ridges and valleys on the southern slope of Poas Volcano. The Rio Poas and Rio Poasito form its eastern border, while the Rio Prendes and Riio Tacares limit the canton to the west. Poas Volcano is the canton&apos;s northernmost point.</obo:IAO_0000115>
        <oboInOwl:hasOBONamespace>GAZ</oboInOwl:hasOBONamespace>
        <oboInOwl:id>GAZ:00068645</oboInOwl:id>
        <rdfs:label>Poas Canton</rdfs:label>
    </owl:NamedIndividual>
    


    <!-- http://purl.obolibrary.org/obo/GAZ_00068646 -->

    <owl:NamedIndividual rdf:about="http://purl.obolibrary.org/obo/GAZ_00068646">
        <obo:RO_0001025 rdf:resource="http://purl.obolibrary.org/obo/GAZ_00003205"/>
        <obo:IAO_0000115>The sixth canton in the province of Alajuela in Costa Rica. The canton covers an area of 126.62 km2. The capital city of the canton is also called Naranjo. The Rio Grande forms the western and southern boundaries of the canton. The Rio Espino is on the north, and the Rio Colorado and Rio Molino establish the eastern border.</obo:IAO_0000115>
        <oboInOwl:hasOBONamespace>GAZ</oboInOwl:hasOBONamespace>
        <oboInOwl:id>GAZ:00068646</oboInOwl:id>
        <rdfs:label>Naranjo Canton</rdfs:label>
    </owl:NamedIndividual>
    


    <!-- http://purl.obolibrary.org/obo/GAZ_00068647 -->

    <owl:NamedIndividual rdf:about="http://purl.obolibrary.org/obo/GAZ_00068647">
        <obo:RO_0001025 rdf:resource="http://purl.obolibrary.org/obo/GAZ_00003205"/>
        <obo:IAO_0000115>The 14th canton in the province of Alajuela in Costa Rica. The canton covers an area of 1,358.86 km2. The capital city of the canton is also called Los Chiles. The canton lies along the border of Nicaragua at the top of the Llanura de San Carlos (San Carlos Plain) in north central Costa Rica. The Rio Pocosol forms the southeastern boundary of the canton, with (from north to south) the Rio Rita, Rio Monico, Riio Frio and the Rio Purgatorio establishing the southwestern border.</obo:IAO_0000115>
        <oboInOwl:hasOBONamespace>GAZ</oboInOwl:hasOBONamespace>
        <oboInOwl:id>GAZ:00068647</oboInOwl:id>
        <rdfs:label>Los Chiles Canton</rdfs:label>
    </owl:NamedIndividual>
    


    <!-- http://purl.obolibrary.org/obo/GAZ_00068648 -->

    <owl:NamedIndividual rdf:about="http://purl.obolibrary.org/obo/GAZ_00068648">
        <obo:RO_0001025 rdf:resource="http://purl.obolibrary.org/obo/GAZ_00003205"/>
        <obo:IAO_0000115>The third canton in the province of Alajuela in Costa Rica. The canton covers an area of 395.72 km2. The capital city of the canton is also called Grecia. The canton lies among ridges and valleys on the southwestern slope of Poas Volcano. One area is completely separated from the remainder of the canton by the Cordillera Central (Central Mountain Range). Known as Rio Cuarto, this area lies on the Caribbean Plain, and is intended to form its own canton at some unspecified future date. The Rio Poas and the Rio Prendes establish a large portion of the eastern border of the elongated canton, with the Rio Sarchi serving the same purpose on its the western edge. The Rio Grande is the southern border.</obo:IAO_0000115>
        <oboInOwl:hasOBONamespace>GAZ</oboInOwl:hasOBONamespace>
        <oboInOwl:id>GAZ:00068648</oboInOwl:id>
        <rdfs:label>Grecia Canton</rdfs:label>
    </owl:NamedIndividual>
    


    <!-- http://purl.obolibrary.org/obo/GAZ_00068649 -->

    <owl:NamedIndividual rdf:about="http://purl.obolibrary.org/obo/GAZ_00068649">
        <obo:RO_0001025 rdf:resource="http://purl.obolibrary.org/obo/GAZ_00003205"/>
        <obo:IAO_0000115>The 15th canton in the province of Alajuela in Costa Rica. The canton covers an area of 758.32 km2. The capital city of the canton is San Rafael de Guatuso. It is a diamond-shaped canton, with the Rio Purgatorio and the Rio Frio as the northeast border, the Rio Cucaracha as a portion of the southeast border, the Cordillera de Guanacaste on the southwest border, and the Rio Rito and the Rio Monico on the northwest. Tenorio Volcano marks the far western point of the canton.</obo:IAO_0000115>
        <oboInOwl:hasOBONamespace>GAZ</oboInOwl:hasOBONamespace>
        <oboInOwl:id>GAZ:00068649</oboInOwl:id>
        <rdfs:label>Guatuso Canton</rdfs:label>
    </owl:NamedIndividual>
    


    <!-- http://purl.obolibrary.org/obo/GAZ_00068650 -->

    <owl:NamedIndividual rdf:about="http://purl.obolibrary.org/obo/GAZ_00068650">
        <obo:RO_0001025 rdf:resource="http://purl.obolibrary.org/obo/GAZ_00003205"/>
        <obo:IAO_0000115>The fourth canton in the province of Alajuela in Costa Rica. The canton covers an area of 125.90 km2. The capital city of the canton is also called San Mateo. The northern border of the elongated province is formed by the Rio Jesus Maria, Rio Machuca, Rio Agua Agria, Rio Calera and Quebrada Zapote. The Quebrada Concepcion, Rio Grande de Tarcoles and the Rio Machuca establish the southern border. Cerro La Lana is a landmark that delineates a northeast tip of the canton.</obo:IAO_0000115>
        <oboInOwl:hasOBONamespace>GAZ</oboInOwl:hasOBONamespace>
        <oboInOwl:id>GAZ:00068650</oboInOwl:id>
        <rdfs:label>San Mateo Canton</rdfs:label>
    </owl:NamedIndividual>
    


    <!-- http://purl.obolibrary.org/obo/GAZ_00068651 -->

    <owl:NamedIndividual rdf:about="http://purl.obolibrary.org/obo/GAZ_00068651">
        <obo:RO_0001025 rdf:resource="http://purl.obolibrary.org/obo/GAZ_00003205"/>
        <obo:IAO_0000115>The seventh canton in the province of Alajuela in Costa Rica. The canton covers an area of 38.06 km2. The capital city of the canton is also called Palmares. The canton encompasses a circular area with the city of Palmares at its center. The Montes de Aguacate establish the boundary on the canton&apos;s southwestern edge and the Rio Grande delineates the boundary on its north and northeast sides.</obo:IAO_0000115>
        <oboInOwl:hasOBONamespace>GAZ</oboInOwl:hasOBONamespace>
        <oboInOwl:id>GAZ:00068651</oboInOwl:id>
        <rdfs:label>Palmares Canton</rdfs:label>
    </owl:NamedIndividual>
    


    <!-- http://purl.obolibrary.org/obo/GAZ_00068652 -->

    <owl:NamedIndividual rdf:about="http://purl.obolibrary.org/obo/GAZ_00068652">
        <obo:RO_0001025 rdf:resource="http://purl.obolibrary.org/obo/GAZ_00003205"/>
        <obo:IAO_0000115>The second canton in the province of Alajuela in Costa Rica. The canton covers an area of 1,018.64 km2. The capital city of the canton is also called San Ramon. An oddly-shaped canton, San Ramon stretches north through the eastern heights of the Cordillera de Tilaran, looking down on the Central Valley (Valle Central) to its east. The canton forms the border with the province of Guanacaste to the west.</obo:IAO_0000115>
        <oboInOwl:hasOBONamespace>GAZ</oboInOwl:hasOBONamespace>
        <oboInOwl:id>GAZ:00068652</oboInOwl:id>
        <rdfs:label>San Ramon Canton</rdfs:label>
    </owl:NamedIndividual>
    


    <!-- http://purl.obolibrary.org/obo/GAZ_00068653 -->

    <owl:NamedIndividual rdf:about="http://purl.obolibrary.org/obo/GAZ_00068653">
        <obo:RO_0001025 rdf:resource="http://purl.obolibrary.org/obo/GAZ_00003205"/>
        <obo:IAO_0000115>The 12th canton in the province of Alajuela in Costa Rica. The canton covers an area of 120.25 km2. The capital city of the canton is Sarchi Norte. The elongated canton lies between the Rio Molina and Rio Toro on the northwest and the Rio Sarchi on the southeast. It reaches northward into the high valley of the Cordillera Central between the Poas and Platanar volcanoes.</obo:IAO_0000115>
        <oboInOwl:hasOBONamespace>GAZ</oboInOwl:hasOBONamespace>
        <oboInOwl:id>GAZ:00068653</oboInOwl:id>
        <rdfs:label>Valverde Vega Canton</rdfs:label>
    </owl:NamedIndividual>
    


    <!-- http://purl.obolibrary.org/obo/GAZ_00068654 -->

    <owl:NamedIndividual rdf:about="http://purl.obolibrary.org/obo/GAZ_00068654">
        <obo:RO_0001025 rdf:resource="http://purl.obolibrary.org/obo/GAZ_00003205"/>
        <obo:IAO_0000115>The fifth canton in the province of Alajuela in Costa Rica. The canton covers an area of 127.19 km2. The capital city of the canton is also called Atenas. It is a fairly compact canton, mountainous for the most part. The Rio Grande forms the border on the canton&apos;s north and east sides. As the river moves south, it is joined by two other large rivers, the Rio Poas and the Rio Virilla, before turning west again and forming the canton&apos;s southern border under a new name, the Rio Grande de Tarcoles. The western border of the canton is established by a series of quebradas (canyons) that cut through the Coastal Mountain Range.</obo:IAO_0000115>
        <oboInOwl:hasOBONamespace>GAZ</oboInOwl:hasOBONamespace>
        <oboInOwl:id>GAZ:00068654</oboInOwl:id>
        <rdfs:label>Atenas Canton</rdfs:label>
    </owl:NamedIndividual>
    


    <!-- http://purl.obolibrary.org/obo/GAZ_00068655 -->

    <owl:NamedIndividual rdf:about="http://purl.obolibrary.org/obo/GAZ_00068655">
        <rdf:type rdf:resource="http://purl.obolibrary.org/obo/ENVO_00000106"/>
        <obo:RO_0001025 rdf:resource="http://purl.obolibrary.org/obo/GAZ_00068660"/>
        <obo:IAO_0000115>A range of mountains in Costa Rica, part of the Continental Divide east of Lake Arenal and the nearby active volcano Arenal, and running into the Cordillera Central range further east. It is located in the Abangares district of the province of Guanacaste.</obo:IAO_0000115>
        <oboInOwl:hasOBONamespace>GAZ</oboInOwl:hasOBONamespace>
        <oboInOwl:id>GAZ:00068655</oboInOwl:id>
        <rdfs:label>Cordillera de Tilaran</rdfs:label>
    </owl:NamedIndividual>
    


    <!-- http://purl.obolibrary.org/obo/GAZ_00068656 -->

    <owl:NamedIndividual rdf:about="http://purl.obolibrary.org/obo/GAZ_00068656">
        <obo:RO_0001025 rdf:resource="http://purl.obolibrary.org/obo/GAZ_00003205"/>
        <obo:IAO_0000115>The 13th canton in the province of Alajuela in Costa Rica. The canton covers an area of 1,580.67 km2. The capital city of the canton is also called Upala. Upala Canton is bordered by Nicaragua on the north, the Rio Las Haciendas on the northwest, Rio Rito on the southeast, and the Cordillera de Guanacaste on the south. The Rincon de la Vieja, Santa Maria, Miravalles and Tenorio volcanoes are landmarks along the southern border.</obo:IAO_0000115>
        <oboInOwl:hasOBONamespace>GAZ</oboInOwl:hasOBONamespace>
        <oboInOwl:id>GAZ:00068656</oboInOwl:id>
        <rdfs:label>Upala Canton</rdfs:label>
    </owl:NamedIndividual>
    


    <!-- http://purl.obolibrary.org/obo/GAZ_00068657 -->

    <owl:NamedIndividual rdf:about="http://purl.obolibrary.org/obo/GAZ_00068657">
        <obo:RO_0001025 rdf:resource="http://purl.obolibrary.org/obo/GAZ_00003205"/>
        <obo:IAO_0000115>The ninth canton in the province of Alajuela in Costa Rica. The canton covers an area of 141.92 km2. The capital city of the canton is also called Orotina. The canton lies on the western side of the Coastal Mountain Range between the Rio Jesus Maria and Rio Machuca on the north and the Rio Grande de Tarcoles on the south.</obo:IAO_0000115>
        <oboInOwl:hasOBONamespace>GAZ</oboInOwl:hasOBONamespace>
        <oboInOwl:id>GAZ:00068657</oboInOwl:id>
        <rdfs:label>Orotina Canton</rdfs:label>
    </owl:NamedIndividual>
    


    <!-- http://purl.obolibrary.org/obo/GAZ_00068658 -->

    <owl:NamedIndividual rdf:about="http://purl.obolibrary.org/obo/GAZ_00068658">
        <obo:RO_0001025 rdf:resource="http://purl.obolibrary.org/obo/GAZ_00003205"/>
        <obo:IAO_0000115>The first canton in the province of Alajuela in Costa Rica. Its capital is the provincial capital city of Alajuela. Northward from the city of Alajuela, the canton continues along the border with the province of Heredia to its east, encompassing a strip of the Cordillera Central (Central Mountain Range) between Poas Volcano and Barva Volcano. On the Caribbean side of the mountains, the canton takes in a portion of the Sarapiqui area. The Rio Poas (Poas River) forms the major portion of the canton&apos;s western border, finally giving way to the Rio Poasito as the territory ascends into the Cordillera Central.</obo:IAO_0000115>
        <oboInOwl:hasOBONamespace>GAZ</oboInOwl:hasOBONamespace>
        <oboInOwl:id>GAZ:00068658</oboInOwl:id>
        <rdfs:label>Alajuela Canton</rdfs:label>
    </owl:NamedIndividual>
    


    <!-- http://purl.obolibrary.org/obo/GAZ_00068659 -->

    <owl:NamedIndividual rdf:about="http://purl.obolibrary.org/obo/GAZ_00068659">
        <obo:RO_0001025 rdf:resource="http://purl.obolibrary.org/obo/GAZ_00003205"/>
        <obo:IAO_0000115>The 11th canton in the province of Alajuela in Costa Rica. The canton covers an area of 155.33 km2. The capital city of the canton is Zarcero. It is a diamond-shaped canton, with the Rio Espina as the border on the northwest and the southwest sides. The Rio Toro forms the southeastern border, and the Rio La Vieja borders the northeast.</obo:IAO_0000115>
        <oboInOwl:hasOBONamespace>GAZ</oboInOwl:hasOBONamespace>
        <oboInOwl:id>GAZ:00068659</oboInOwl:id>
        <rdfs:label>Alfaro Ruiz Canton</rdfs:label>
    </owl:NamedIndividual>
    


    <!-- http://purl.obolibrary.org/obo/GAZ_00068660 -->

    <owl:NamedIndividual rdf:about="http://purl.obolibrary.org/obo/GAZ_00068660">
        <obo:RO_0001025 rdf:resource="http://purl.obolibrary.org/obo/GAZ_00003210"/>
        <obo:IAO_0000115>The seventh canton in the province of Guanacaste in Costa Rica. The canton covers an area of 675.76 km2. Its capital city is Las Juntas. The canton begins on the coastline of the Gulf of Nicoya north of the mouth of the Rio Abangares. It widens between the Rio Lajas on the northwest and Rio Lagartos on the east as it reaches up into the Cordillera de Tilaran.</obo:IAO_0000115>
        <oboInOwl:hasOBONamespace>GAZ</oboInOwl:hasOBONamespace>
        <oboInOwl:id>GAZ:00068660</oboInOwl:id>
        <rdfs:label>Abangares Canton</rdfs:label>
    </owl:NamedIndividual>
    


    <!-- http://purl.obolibrary.org/obo/GAZ_00068661 -->

    <owl:NamedIndividual rdf:about="http://purl.obolibrary.org/obo/GAZ_00068661">
        <rdf:type rdf:resource="http://purl.obolibrary.org/obo/ENVO_00000004"/>
        <obo:RO_0001025 rdf:resource="http://purl.obolibrary.org/obo/GAZ_00068651"/>
        <obo:IAO_0000115>A district of Palmares Canton.</obo:IAO_0000115>
        <oboInOwl:hasOBONamespace>GAZ</oboInOwl:hasOBONamespace>
        <oboInOwl:id>GAZ:00068661</oboInOwl:id>
        <rdfs:label>Montes de Aguacate District</rdfs:label>
    </owl:NamedIndividual>
    


    <!-- http://purl.obolibrary.org/obo/GAZ_00068662 -->

    <owl:NamedIndividual rdf:about="http://purl.obolibrary.org/obo/GAZ_00068662">
        <obo:RO_0001025 rdf:resource="http://purl.obolibrary.org/obo/GAZ_00003211"/>
        <obo:IAO_0000115>The fourth canton in the province of Cartago in Costa Rica. The canton covers an area of 286.43 km2. The capital city of the canton is Juan Vinas. The Rio Turrialba forms the northern boundary of the canton of Jimenez, with the Rio Reventazon and Rio Atirro establishing the eastern border and the Rio Pejibaye delineating a major portion of the canton&apos;s border on the west.</obo:IAO_0000115>
        <oboInOwl:hasOBONamespace>GAZ</oboInOwl:hasOBONamespace>
        <oboInOwl:id>GAZ:00068662</oboInOwl:id>
        <rdfs:label>Jimenez Canton</rdfs:label>
    </owl:NamedIndividual>
    


    <!-- http://purl.obolibrary.org/obo/GAZ_00068663 -->

    <owl:NamedIndividual rdf:about="http://purl.obolibrary.org/obo/GAZ_00068663">
        <obo:RO_0001025 rdf:resource="http://purl.obolibrary.org/obo/GAZ_00003211"/>
        <obo:IAO_0000115>The sixth canton in the province of Cartago in Costa Rica. The canton covers an area of 81.06 km2. The capital city of the canton is Pacayas. The defunct Caribbean railway line delineates a portion of the southern boundary of the oval-shaped canton, along with the Rio Reventazon. The Rio Turrialba on the east and the Rio Birris on the west help establish the canton&apos;s northern limits, which reach into the Cordillera Central.</obo:IAO_0000115>
        <oboInOwl:hasOBONamespace>GAZ</oboInOwl:hasOBONamespace>
        <oboInOwl:id>GAZ:00068663</oboInOwl:id>
        <rdfs:label>Alvarado Canton</rdfs:label>
    </owl:NamedIndividual>
    


    <!-- http://purl.obolibrary.org/obo/GAZ_00068664 -->

    <owl:NamedIndividual rdf:about="http://purl.obolibrary.org/obo/GAZ_00068664">
        <obo:RO_0001025 rdf:resource="http://purl.obolibrary.org/obo/GAZ_00003211"/>
        <obo:IAO_0000115>The eighth canton in the province of Cartago in Costa Rica. The canton covers an area of 167.69 km2. The capital city of the canton is El Tejar. El Guarco is an elongated canton that stretches southeast from its capital city to encompass a swatch of the Cordillera de Talamanca. The Carretera Interamericana (Pan-American Highway) delineates the canton&apos;s lengthy southwestern border.</obo:IAO_0000115>
        <oboInOwl:hasOBONamespace>GAZ</oboInOwl:hasOBONamespace>
        <oboInOwl:id>GAZ:00068664</oboInOwl:id>
        <rdfs:label>El Guarco Canton</rdfs:label>
    </owl:NamedIndividual>
    


    <!-- http://purl.obolibrary.org/obo/GAZ_00068665 -->

    <owl:NamedIndividual rdf:about="http://purl.obolibrary.org/obo/GAZ_00068665">
        <obo:RO_0001025 rdf:resource="http://purl.obolibrary.org/obo/GAZ_00003211"/>
        <obo:IAO_0000115>The third canton in the province of Cartago in Costa Rica. The canton covers an area of 44.83 km2. The capital city of the canton is Tres Rios. La Union is a compact canton situation midway between the national capital of San Jose and the former colonial capital city of Cartago.</obo:IAO_0000115>
        <oboInOwl:hasOBONamespace>GAZ</oboInOwl:hasOBONamespace>
        <oboInOwl:id>GAZ:00068665</oboInOwl:id>
        <rdfs:label>La Union Canton</rdfs:label>
    </owl:NamedIndividual>
    


    <!-- http://purl.obolibrary.org/obo/GAZ_00068666 -->

    <owl:NamedIndividual rdf:about="http://purl.obolibrary.org/obo/GAZ_00068666">
        <obo:RO_0001025 rdf:resource="http://purl.obolibrary.org/obo/GAZ_00003211"/>
        <obo:IAO_0000115>The first canton in the province of Cartago in Costa Rica. The canton covers an area of 287.77 km2. Its capital is the provincial capital city of Cartago. Cartago is a T-shaped canton stretching southeast from its capital city to encompass a thin swatch of the Cordillera de Talamanca (Talamanca Mountain Range).</obo:IAO_0000115>
        <oboInOwl:hasOBONamespace>GAZ</oboInOwl:hasOBONamespace>
        <oboInOwl:id>GAZ:00068666</oboInOwl:id>
        <rdfs:label>Cartago Canton</rdfs:label>
    </owl:NamedIndividual>
    


    <!-- http://purl.obolibrary.org/obo/GAZ_00068667 -->

    <owl:NamedIndividual rdf:about="http://purl.obolibrary.org/obo/GAZ_00068667">
        <obo:RO_0001025 rdf:resource="http://purl.obolibrary.org/obo/GAZ_00003211"/>
        <obo:IAO_0000115>The second canton in the province of Cartago in Costa Rica. The canton covers an area of 411.91 km2, The capital city of the canton is also called Paraiso. Paraiso is an elongated canton that stretches southeast from its capital city to encompass a swatch of the Cordillera de Talamanca.</obo:IAO_0000115>
        <oboInOwl:hasOBONamespace>GAZ</oboInOwl:hasOBONamespace>
        <oboInOwl:id>GAZ:00068667</oboInOwl:id>
        <rdfs:label>Paraiso Canton</rdfs:label>
    </owl:NamedIndividual>
    


    <!-- http://purl.obolibrary.org/obo/GAZ_00068668 -->

    <owl:NamedIndividual rdf:about="http://purl.obolibrary.org/obo/GAZ_00068668">
        <obo:RO_0001025 rdf:resource="http://purl.obolibrary.org/obo/GAZ_00003211"/>
        <obo:IAO_0000115>The seventh canton in the province of Cartago in Costa Rica. The canton covers an area of 202.31 km2. The capital city of the canton is San Rafael. The canton extends from its suburban capital city of San Rafael northward into the Cordillera Central. Irazu Volcano looms large in the northern reaches of the canton.</obo:IAO_0000115>
        <oboInOwl:hasOBONamespace>GAZ</oboInOwl:hasOBONamespace>
        <oboInOwl:id>GAZ:00068668</oboInOwl:id>
        <rdfs:label>Oreamuno Canton</rdfs:label>
    </owl:NamedIndividual>
    


    <!-- http://purl.obolibrary.org/obo/GAZ_00068669 -->

    <owl:NamedIndividual rdf:about="http://purl.obolibrary.org/obo/GAZ_00068669">
        <obo:RO_0001025 rdf:resource="http://purl.obolibrary.org/obo/GAZ_00003210"/>
        <obo:IAO_0000115>The ninth canton in the province of Guanacaste in Costa Rica. The canton covers an area of 565.59 km2. Its capital city is Carmona. The canton encompasses a piece of the coastline of the Gulf of Nicoya near the mouth of the Rio Tempisque, including Isla Berrugate. It cuts across the center of the Nicoya Peninsula to the Pacific coast between the Rio Ora to the north and the Rio Bongo to the south.</obo:IAO_0000115>
        <oboInOwl:hasOBONamespace>GAZ</oboInOwl:hasOBONamespace>
        <oboInOwl:id>GAZ:00068669</oboInOwl:id>
        <rdfs:label>Nandayure Canton</rdfs:label>
    </owl:NamedIndividual>
    


    <!-- http://purl.obolibrary.org/obo/GAZ_00068670 -->

    <owl:NamedIndividual rdf:about="http://purl.obolibrary.org/obo/GAZ_00068670">
        <obo:RO_0001025 rdf:resource="http://purl.obolibrary.org/obo/GAZ_00003210"/>
        <obo:IAO_0000115>The tenth canton in the province of Guanacaste in Costa Rica. The canton covers an area of 1,383.90 km2. Its capital city is also called La Cruz. The canton is the northernmost in the country. It encompasses the Pacific coastline from the border with Nicaragua as far south as Bahia Nancite, including the Peninsula de Santa Elena.</obo:IAO_0000115>
        <oboInOwl:hasOBONamespace>GAZ</oboInOwl:hasOBONamespace>
        <oboInOwl:id>GAZ:00068670</oboInOwl:id>
        <rdfs:label>La Cruz Canton</rdfs:label>
    </owl:NamedIndividual>
    


    <!-- http://purl.obolibrary.org/obo/GAZ_00068671 -->

    <owl:NamedIndividual rdf:about="http://purl.obolibrary.org/obo/GAZ_00068671">
        <obo:RO_0001025 rdf:resource="http://purl.obolibrary.org/obo/GAZ_00003210"/>
        <obo:IAO_0000115>The fifth canton in the province of Guanacaste in Costa Rica. The canton covers an area of 577.54 km2. Its capital city is Filadelfia. The canton is shaped like a boot, with the Pacific Ocean at the top. The Rio Tempisque decorates the front of the boot from top to toe. The Rio Canas and Rio Bolson provide the heel and sole.</obo:IAO_0000115>
        <oboInOwl:hasOBONamespace>GAZ</oboInOwl:hasOBONamespace>
        <oboInOwl:id>GAZ:00068671</oboInOwl:id>
        <rdfs:label>Carrillo Canton</rdfs:label>
    </owl:NamedIndividual>
    


    <!-- http://purl.obolibrary.org/obo/GAZ_00068672 -->

    <owl:NamedIndividual rdf:about="http://purl.obolibrary.org/obo/GAZ_00068672">
        <obo:RO_0001025 rdf:resource="http://purl.obolibrary.org/obo/GAZ_00003210"/>
        <obo:IAO_0000115>The third canton in the province of Guanacaste in Costa Rica. The canton covers an area of 1,312.27 km2. Its capital city is also called Santa Cruz. The heart-shaped canton is on the northern Pacific coast between Bahia Potrero to the north and the mouth of the Rio Montana to the south. It includes Cabo Velas, the furthermost western point on the Nicoya Peninsula. The Rio Tempisque delineates a small portion of the eastern border.</obo:IAO_0000115>
        <oboInOwl:hasOBONamespace>GAZ</oboInOwl:hasOBONamespace>
        <oboInOwl:id>GAZ:00068672</oboInOwl:id>
        <rdfs:label>Santa Cruz Canton</rdfs:label>
    </owl:NamedIndividual>
    


    <!-- http://purl.obolibrary.org/obo/GAZ_00068673 -->

    <owl:NamedIndividual rdf:about="http://purl.obolibrary.org/obo/GAZ_00068673">
        <obo:RO_0001025 rdf:resource="http://purl.obolibrary.org/obo/GAZ_00003210"/>
        <obo:IAO_0000115>The sixth canton in the province of Guanacaste in Costa Rica. The canton covers an area of 682.20 km2. Its capital city is also called Canas. The elongated canton touches the Rio Tempisque in the southwest. It keeps the Rio Bebedero and Roo Tenorio on its western boundary as it widens to encompass agricultural lowlands before climbing into the Cordillera de Guanacaste up to the Tenorio Volcano National Park.</obo:IAO_0000115>
        <oboInOwl:hasOBONamespace>GAZ</oboInOwl:hasOBONamespace>
        <oboInOwl:id>GAZ:00068673</oboInOwl:id>
        <rdfs:label>Canas Canton</rdfs:label>
    </owl:NamedIndividual>
    


    <!-- http://purl.obolibrary.org/obo/GAZ_00068674 -->

    <owl:NamedIndividual rdf:about="http://purl.obolibrary.org/obo/GAZ_00068674">
        <obo:RO_0001025 rdf:resource="http://purl.obolibrary.org/obo/GAZ_00003210"/>
        <obo:IAO_0000115>The eighth canton in the province of Guanacaste in Costa Rica. The canton covers an area of 638.39 km2. Its capital city is also called Tilaran. The canton surrounds Lake Arenal (Laguna de Arenal) except for the lake&apos;s southeast end, which belongs to the province of Alajuela. The northern border is in the Cordillera de Guanacaste, touching the Rio Corobici at its northernmost limits. The south part of the canton is in the Cordillera de Tilaran.</obo:IAO_0000115>
        <oboInOwl:hasOBONamespace>GAZ</oboInOwl:hasOBONamespace>
        <oboInOwl:id>GAZ:00068674</oboInOwl:id>
        <rdfs:label>Tilaran Canton</rdfs:label>
    </owl:NamedIndividual>
    


    <!-- http://purl.obolibrary.org/obo/GAZ_00068675 -->

    <owl:NamedIndividual rdf:about="http://purl.obolibrary.org/obo/GAZ_00068675">
        <obo:RO_0001025 rdf:resource="http://purl.obolibrary.org/obo/GAZ_00003210"/>
        <obo:IAO_0000115>The fourth canton in the province of Guanacaste in Costa Rica. The canton covers an area of 1,273.49 km2. Its capital city is also called Bagaces. The Rii Salto on the west and Rio Tenorio on the east delineate this canton, with the Rio Tempisque as the southern border and the northern border high in the Cordillera de Guanacaste. Miravalles Volcano sits near that border&apos;s midway point.</obo:IAO_0000115>
        <oboInOwl:hasOBONamespace>GAZ</oboInOwl:hasOBONamespace>
        <oboInOwl:id>GAZ:00068675</oboInOwl:id>
        <rdfs:label>Bagaces Canton</rdfs:label>
    </owl:NamedIndividual>
    


    <!-- http://purl.obolibrary.org/obo/GAZ_00068676 -->

    <owl:NamedIndividual rdf:about="http://purl.obolibrary.org/obo/GAZ_00068676">
        <obo:RO_0001025 rdf:resource="http://purl.obolibrary.org/obo/GAZ_00003210"/>
        <obo:IAO_0000115>The 11th canton in the province of Guanacaste in Costa Rica. The canton covers an area of 261.42 km2. Its capital city is also called Hojancha. The canton is in the midsection of the Nicoya Peninsula. It is relatively compact, with a single tentacle reaching south to encompass a small portion of the Pacific coastline from Playa Carrillo southward to the mouth of the Rio Ora.</obo:IAO_0000115>
        <oboInOwl:hasOBONamespace>GAZ</oboInOwl:hasOBONamespace>
        <oboInOwl:id>GAZ:00068676</oboInOwl:id>
        <rdfs:label>Hojancha Canton</rdfs:label>
    </owl:NamedIndividual>
    


    <!-- http://purl.obolibrary.org/obo/GAZ_00068677 -->

    <owl:NamedIndividual rdf:about="http://purl.obolibrary.org/obo/GAZ_00068677">
        <obo:RO_0001025 rdf:resource="http://purl.obolibrary.org/obo/GAZ_00003210"/>
        <obo:IAO_0000115>The first canton in the province of Guanacaste in Costa Rica. The canton covers an area of 1,436.47 km2. Cerro Cacao and Rincon de la Vieja Volcano National Park mark the northeast border of this diamond-shaped canton. The Rio Salto delineates the southwestern border as far as the Rio Tempisque, and the Tempisque forms the border on the southeast as far as the Bahia Naranjo. The canton includes the most visited portion of Santa Rosa National Park on its northwest border.</obo:IAO_0000115>
        <oboInOwl:hasOBONamespace>GAZ</oboInOwl:hasOBONamespace>
        <oboInOwl:id>GAZ:00068677</oboInOwl:id>
        <rdfs:label>Liberia Canton</rdfs:label>
    </owl:NamedIndividual>
    


    <!-- http://purl.obolibrary.org/obo/GAZ_00068678 -->

    <owl:NamedIndividual rdf:about="http://purl.obolibrary.org/obo/GAZ_00068678">
        <obo:RO_0001025 rdf:resource="http://purl.obolibrary.org/obo/GAZ_00003210"/>
        <obo:IAO_0000115>The second canton in the province of Guanacaste in Costa Rica. The canton covers an area of 1,333.68 km2. Its capital city is also called Nicoya. The Rio Tempisque establishes the northeast boundary of the canton, which cuts through the midsection of the Nicoya Peninsula, touching the Gulf of Nicoya on the east before curving southward to the Pacific Ocean.</obo:IAO_0000115>
        <oboInOwl:hasOBONamespace>GAZ</oboInOwl:hasOBONamespace>
        <oboInOwl:id>GAZ:00068678</oboInOwl:id>
        <rdfs:label>Nicoya Canton</rdfs:label>
    </owl:NamedIndividual>
    


    <!-- http://purl.obolibrary.org/obo/GAZ_00068679 -->

    <owl:NamedIndividual rdf:about="http://purl.obolibrary.org/obo/GAZ_00068679">
        <obo:RO_0001025 rdf:resource="http://purl.obolibrary.org/obo/GAZ_00003208"/>
        <obo:IAO_0000115>The seventh canton in the province of Heredia in Costa Rica. The canton covers an area of 12.15 km2. The capital city of the canton is San Antonio. The compact canton is on the western side of the General Canas Freeway (Autopista General Canas) midway between the national capital city of San Jose and the Juan Santamaria International Airport.</obo:IAO_0000115>
        <oboInOwl:hasOBONamespace>GAZ</oboInOwl:hasOBONamespace>
        <oboInOwl:id>GAZ:00068679</oboInOwl:id>
        <rdfs:label>Belen Canton</rdfs:label>
    </owl:NamedIndividual>
    


    <!-- http://purl.obolibrary.org/obo/GAZ_00068680 -->

    <owl:NamedIndividual rdf:about="http://purl.obolibrary.org/obo/GAZ_00068680">
        <obo:RO_0001025 rdf:resource="http://purl.obolibrary.org/obo/GAZ_00003208"/>
        <obo:IAO_0000115>The tenth canton in the province of Heredia in Costa Rica. The canton covers an area of 2,140.54 km2. The capital city of the canton is Puerto Viejo. The canton includes the major portion of the Sarapiqui region, and is named for its major waterway, the Rio Sarapiqui, which forms the canton&apos;s eastern border. The western half of the canton gives way to the San Carlos Plain (Llanura de San Carlos). Heredia&apos;s provincial border with Alajuela, which runs through the middle of the San Carlos Plain, marks the canton&apos;s western limit. The southern boundary of the canton is established by the Rio Virgen.</obo:IAO_0000115>
        <oboInOwl:hasOBONamespace>GAZ</oboInOwl:hasOBONamespace>
        <oboInOwl:id>GAZ:00068680</oboInOwl:id>
        <rdfs:label>Sarapiqui Canton</rdfs:label>
    </owl:NamedIndividual>
    


    <!-- http://purl.obolibrary.org/obo/GAZ_00068681 -->

    <owl:NamedIndividual rdf:about="http://purl.obolibrary.org/obo/GAZ_00068681">
        <obo:RO_0001025 rdf:resource="http://purl.obolibrary.org/obo/GAZ_00003209"/>
        <obo:RO_0001025 rdf:resource="http://purl.obolibrary.org/obo/GAZ_00003210"/>
        <obo:IAO_0000115>A peninsula on the Pacific coast of Costa Rica and lies in the Guanacaste Province in the north, and the Puntarenas Province in the south. It varies from 19 to 37 miles wide and is approximately 75 miles long, and forms the largest peninsula in the country. It is known for its beaches and is a popular tourist destination.</obo:IAO_0000115>
        <oboInOwl:hasOBONamespace>GAZ</oboInOwl:hasOBONamespace>
        <oboInOwl:id>GAZ:00068681</oboInOwl:id>
        <rdfs:label>Nicoya Peninsula</rdfs:label>
    </owl:NamedIndividual>
    


    <!-- http://purl.obolibrary.org/obo/GAZ_00068682 -->

    <owl:NamedIndividual rdf:about="http://purl.obolibrary.org/obo/GAZ_00068682">
        <obo:RO_0001025 rdf:resource="http://purl.obolibrary.org/obo/GAZ_00002901"/>
        <obo:IAO_0000115>An administrative area which is managed by the Sistema Nacional de Areas de Conservacion for the purposes of conservation in the western part of Costa Rica, including the Tempisque River valley and the Nicoya Peninsula. It contains a number of National Parks, Wildlife refuges and Forest Reserves.</obo:IAO_0000115>
        <oboInOwl:hasOBONamespace>GAZ</oboInOwl:hasOBONamespace>
        <oboInOwl:id>GAZ:00068682</oboInOwl:id>
        <rdfs:label>Tempisque Conservation Area</rdfs:label>
    </owl:NamedIndividual>
    


    <!-- http://purl.obolibrary.org/obo/GAZ_00068683 -->

    <owl:NamedIndividual rdf:about="http://purl.obolibrary.org/obo/GAZ_00068683">
        <obo:RO_0001025 rdf:resource="http://purl.obolibrary.org/obo/GAZ_00068681"/>
        <obo:RO_0001025 rdf:resource="http://purl.obolibrary.org/obo/GAZ_00068682"/>
        <obo:IAO_0000115>A nature reserve of Costa Rica, part of the Tempisque Conservation Area in the province of Puntarenas, covering an area of 13 km2 terrestrial and 18 km2 marine on the southern tip of the Nicoya Peninsula near Mal Pais.</obo:IAO_0000115>
        <oboInOwl:hasOBONamespace>GAZ</oboInOwl:hasOBONamespace>
        <oboInOwl:id>GAZ:00068683</oboInOwl:id>
        <rdfs:label>Cabo Blanco Absolute Natural Reserve</rdfs:label>
    </owl:NamedIndividual>
    


    <!-- http://purl.obolibrary.org/obo/GAZ_00068684 -->

    <owl:NamedIndividual rdf:about="http://purl.obolibrary.org/obo/GAZ_00068684">
        <obo:RO_0001025 rdf:resource="http://purl.obolibrary.org/obo/GAZ_00068681"/>
        <obo:RO_0001025 rdf:resource="http://purl.obolibrary.org/obo/GAZ_00068682"/>
        <obo:IAO_0000115>A wildlife refuge of Costa Rica, part of the Tempisque Conservation Area, on the Pacific Coast of the Nicoya Peninsula.</obo:IAO_0000115>
        <oboInOwl:hasOBONamespace>GAZ</oboInOwl:hasOBONamespace>
        <oboInOwl:id>GAZ:00068684</oboInOwl:id>
        <rdfs:label>Camaronal Wildlife Refuge</rdfs:label>
    </owl:NamedIndividual>
    


    <!-- http://purl.obolibrary.org/obo/GAZ_00068685 -->

    <owl:NamedIndividual rdf:about="http://purl.obolibrary.org/obo/GAZ_00068685">
        <obo:RO_0001025 rdf:resource="http://purl.obolibrary.org/obo/GAZ_00068681"/>
        <obo:RO_0001025 rdf:resource="http://purl.obolibrary.org/obo/GAZ_00068682"/>
        <obo:IAO_0000115>A wildlife refuge of Costa Rica, part of the Tempisque Conservation Area, and protects tropical forest in the coastal areas of the southern Nicoya Peninsula near Cabuya.</obo:IAO_0000115>
        <oboInOwl:hasOBONamespace>GAZ</oboInOwl:hasOBONamespace>
        <oboInOwl:id>GAZ:00068685</oboInOwl:id>
        <rdfs:label>Cueva Murcielago Wildlife Refuge</rdfs:label>
    </owl:NamedIndividual>
    


    <!-- http://purl.obolibrary.org/obo/GAZ_00068686 -->

    <owl:NamedIndividual rdf:about="http://purl.obolibrary.org/obo/GAZ_00068686">
        <obo:RO_0001025 rdf:resource="http://purl.obolibrary.org/obo/GAZ_00068681"/>
        <obo:RO_0001025 rdf:resource="http://purl.obolibrary.org/obo/GAZ_00068682"/>
        <obo:IAO_0000115>A wildlife refuge of Costa Rica, part of the Tempisque Conservation Area, tropical dry forests on the southern Nicoya Peninsula, near Tambor.</obo:IAO_0000115>
        <oboInOwl:hasOBONamespace>GAZ</oboInOwl:hasOBONamespace>
        <oboInOwl:id>GAZ:00068686</oboInOwl:id>
        <rdfs:label>Curu Wildlife Refuge</rdfs:label>
    </owl:NamedIndividual>
    


    <!-- http://purl.obolibrary.org/obo/GAZ_00068687 -->

    <owl:NamedIndividual rdf:about="http://purl.obolibrary.org/obo/GAZ_00068687">
        <obo:RO_0001025 rdf:resource="http://purl.obolibrary.org/obo/GAZ_00068681"/>
        <obo:RO_0001025 rdf:resource="http://purl.obolibrary.org/obo/GAZ_00068682"/>
        <obo:IAO_0000115>A wildlife refuge in Costa Rica, part of the Tempisque Conservation Area, which protects tropical forest on the Nicoya Peninsula near the small village of San Rafael de Paquera in the Puntarenas Province.</obo:IAO_0000115>
        <oboInOwl:hasOBONamespace>GAZ</oboInOwl:hasOBONamespace>
        <oboInOwl:id>GAZ:00068687</oboInOwl:id>
        <rdfs:label>La Ceiba Wildlife Refuge</rdfs:label>
    </owl:NamedIndividual>
    


    <!-- http://purl.obolibrary.org/obo/GAZ_00068688 -->

    <owl:NamedIndividual rdf:about="http://purl.obolibrary.org/obo/GAZ_00068688">
        <obo:RO_0001025 rdf:resource="http://purl.obolibrary.org/obo/GAZ_00068681"/>
        <obo:RO_0001025 rdf:resource="http://purl.obolibrary.org/obo/GAZ_00068682"/>
        <obo:IAO_0000115>A wildlife refuge in Costa Rica, part of the Tempisque Conservation Area, near Montezuma, Costa Rica on the Nicoya Peninsula.</obo:IAO_0000115>
        <oboInOwl:hasOBONamespace>GAZ</oboInOwl:hasOBONamespace>
        <oboInOwl:id>GAZ:00068688</oboInOwl:id>
        <rdfs:label>Romelia Wildlife Refuge</rdfs:label>
    </owl:NamedIndividual>
    


    <!-- http://purl.obolibrary.org/obo/GAZ_00068689 -->

    <owl:NamedIndividual rdf:about="http://purl.obolibrary.org/obo/GAZ_00068689">
        <obo:RO_0001025 rdf:resource="http://purl.obolibrary.org/obo/GAZ_00068681"/>
        <obo:RO_0001025 rdf:resource="http://purl.obolibrary.org/obo/GAZ_00068682"/>
        <obo:IAO_0000115>A national park of Costa Rica south of Santa Cruz in the Guanacaste Province, and forms part of the Tempisque Conservation Area. It protects both dry and at higher elevations humid tropical forest in the central highlands of the Nicoya Peninsula, including the watersheds of the Diria, Tigre, Verde and Enmedio rivers which have been created a terrain of deep valleys with steep slopes.</obo:IAO_0000115>
        <oboInOwl:hasOBONamespace>GAZ</oboInOwl:hasOBONamespace>
        <oboInOwl:id>GAZ:00068689</oboInOwl:id>
        <rdfs:label>Diria National Park</rdfs:label>
    </owl:NamedIndividual>
    


    <!-- http://purl.obolibrary.org/obo/GAZ_00068690 -->

    <owl:NamedIndividual rdf:about="http://purl.obolibrary.org/obo/GAZ_00068690">
        <obo:IAO_0000115>An inlet of the Pacific Ocean. It separates the Nicoya Peninsula from the mainland of Costa Rica, and encompasses a marine and coastal landscape of wetlands, rocky islands and cliffs.</obo:IAO_0000115>
        <oboInOwl:hasOBONamespace>GAZ</oboInOwl:hasOBONamespace>
        <oboInOwl:id>GAZ:00068690</oboInOwl:id>
        <rdfs:label>Gulf of Nicoya</rdfs:label>
    </owl:NamedIndividual>
    


    <!-- http://purl.obolibrary.org/obo/GAZ_00068691 -->

    <owl:NamedIndividual rdf:about="http://purl.obolibrary.org/obo/GAZ_00068691">
        <obo:RO_0001025 rdf:resource="http://purl.obolibrary.org/obo/GAZ_00003209"/>
        <obo:RO_0001025 rdf:resource="http://purl.obolibrary.org/obo/GAZ_00068690"/>
        <obo:IAO_0000115>An island in the Gulf of Nicoya.</obo:IAO_0000115>
        <oboInOwl:hasOBONamespace>GAZ</oboInOwl:hasOBONamespace>
        <oboInOwl:id>GAZ:00068691</oboInOwl:id>
        <rdfs:label>Isla Venado</rdfs:label>
    </owl:NamedIndividual>
    


    <!-- http://purl.obolibrary.org/obo/GAZ_00068692 -->

    <owl:NamedIndividual rdf:about="http://purl.obolibrary.org/obo/GAZ_00068692">
        <obo:RO_0001025 rdf:resource="http://purl.obolibrary.org/obo/GAZ_00003209"/>
        <obo:RO_0001025 rdf:resource="http://purl.obolibrary.org/obo/GAZ_00068842"/>
        <obo:IAO_0000115>An island in the Gulf of Nicoya.</obo:IAO_0000115>
        <oboInOwl:hasOBONamespace>GAZ</oboInOwl:hasOBONamespace>
        <oboInOwl:id>GAZ:00068692</oboInOwl:id>
        <rdfs:label>Isla San Lucas</rdfs:label>
    </owl:NamedIndividual>
    


    <!-- http://purl.obolibrary.org/obo/GAZ_00068693 -->

    <owl:NamedIndividual rdf:about="http://purl.obolibrary.org/obo/GAZ_00068693">
        <obo:RO_0001025 rdf:resource="http://purl.obolibrary.org/obo/GAZ_00003209"/>
        <obo:RO_0001025 rdf:resource="http://purl.obolibrary.org/obo/GAZ_00068690"/>
        <obo:IAO_0000115>The largest island within mainland Costa Rica. It is located at the upper end of the Gulf of Nicoya.</obo:IAO_0000115>
        <oboInOwl:hasOBONamespace>GAZ</oboInOwl:hasOBONamespace>
        <oboInOwl:id>GAZ:00068693</oboInOwl:id>
        <rdfs:label>Isla Chira</rdfs:label>
    </owl:NamedIndividual>
    


    <!-- http://purl.obolibrary.org/obo/GAZ_00068694 -->

    <owl:NamedIndividual rdf:about="http://purl.obolibrary.org/obo/GAZ_00068694">
        <obo:RO_0001025 rdf:resource="http://purl.obolibrary.org/obo/GAZ_00003209"/>
        <obo:RO_0001025 rdf:resource="http://purl.obolibrary.org/obo/GAZ_00068690"/>
        <obo:IAO_0000115>An island in the Gulf of Nicoya.</obo:IAO_0000115>
        <oboInOwl:hasOBONamespace>GAZ</oboInOwl:hasOBONamespace>
        <oboInOwl:id>GAZ:00068694</oboInOwl:id>
        <rdfs:label>Isla Bejuco</rdfs:label>
    </owl:NamedIndividual>
    


    <!-- http://purl.obolibrary.org/obo/GAZ_00068695 -->

    <owl:NamedIndividual rdf:about="http://purl.obolibrary.org/obo/GAZ_00068695">
        <obo:RO_0001025 rdf:resource="http://purl.obolibrary.org/obo/GAZ_00003209"/>
        <obo:RO_0001025 rdf:resource="http://purl.obolibrary.org/obo/GAZ_00068690"/>
        <obo:IAO_0000115>An island in the Gulf of Nicoya.</obo:IAO_0000115>
        <oboInOwl:hasOBONamespace>GAZ</oboInOwl:hasOBONamespace>
        <oboInOwl:id>GAZ:00068695</oboInOwl:id>
        <rdfs:label>Isla Gitana</rdfs:label>
    </owl:NamedIndividual>
    


    <!-- http://purl.obolibrary.org/obo/GAZ_00068696 -->

    <owl:NamedIndividual rdf:about="http://purl.obolibrary.org/obo/GAZ_00068696">
        <obo:RO_0001025 rdf:resource="http://purl.obolibrary.org/obo/GAZ_00003209"/>
        <obo:RO_0001025 rdf:resource="http://purl.obolibrary.org/obo/GAZ_00068690"/>
        <obo:IAO_0000115>An island in the Gulf of Nicoya.</obo:IAO_0000115>
        <oboInOwl:hasOBONamespace>GAZ</oboInOwl:hasOBONamespace>
        <oboInOwl:id>GAZ:00068696</oboInOwl:id>
        <rdfs:label>Isla Caballo</rdfs:label>
    </owl:NamedIndividual>
    


    <!-- http://purl.obolibrary.org/obo/GAZ_00068697 -->

    <owl:NamedIndividual rdf:about="http://purl.obolibrary.org/obo/GAZ_00068697">
        <obo:RO_0001025 rdf:resource="http://purl.obolibrary.org/obo/GAZ_00003209"/>
        <obo:RO_0001025 rdf:resource="http://purl.obolibrary.org/obo/GAZ_00068690"/>
        <obo:IAO_0000115>Two adjacent islands in the Gulf of Nicoya.</obo:IAO_0000115>
        <oboInOwl:hasOBONamespace>GAZ</oboInOwl:hasOBONamespace>
        <oboInOwl:id>GAZ:00068697</oboInOwl:id>
        <rdfs:label>Islas Tortuga</rdfs:label>
    </owl:NamedIndividual>
    


    <!-- http://purl.obolibrary.org/obo/GAZ_00068698 -->

    <owl:NamedIndividual rdf:about="http://purl.obolibrary.org/obo/GAZ_00068698">
        <obo:RO_0001025 rdf:resource="http://purl.obolibrary.org/obo/GAZ_00068669"/>
        <obo:RO_0001025 rdf:resource="http://purl.obolibrary.org/obo/GAZ_00068690"/>
        <obo:IAO_0000115>An island in the Gulf of Nicoya.</obo:IAO_0000115>
        <oboInOwl:hasOBONamespace>GAZ</oboInOwl:hasOBONamespace>
        <oboInOwl:id>GAZ:00068698</oboInOwl:id>
        <rdfs:label>Isla Berrugate</rdfs:label>
    </owl:NamedIndividual>
    


    <!-- http://purl.obolibrary.org/obo/GAZ_00068699 -->

    <owl:NamedIndividual rdf:about="http://purl.obolibrary.org/obo/GAZ_00068699">
        <obo:RO_0001025 rdf:resource="http://purl.obolibrary.org/obo/GAZ_00002901"/>
        <obo:IAO_0000115>An administrative area which is managed by the Sistema Nacional de Areas de Conservacion for the purposes of conservation in the northwestern part of Costa Rica. It contains three National Parks, as well as wildlife refuges and other nature reserves. The area contains the Area de Conservacion Guanacaste World Heritage Site.</obo:IAO_0000115>
        <oboInOwl:hasOBONamespace>GAZ</oboInOwl:hasOBONamespace>
        <oboInOwl:id>GAZ:00068699</oboInOwl:id>
        <rdfs:label>Guanacaste Conservation Area</rdfs:label>
    </owl:NamedIndividual>
    


    <!-- http://purl.obolibrary.org/obo/GAZ_00068700 -->

    <owl:NamedIndividual rdf:about="http://purl.obolibrary.org/obo/GAZ_00068700">
        <obo:RO_0001025 rdf:resource="http://purl.obolibrary.org/obo/GAZ_00068699"/>
        <obo:IAO_0000115>A part of the Guanacaste Conservation Area and the Area de Conservacion Guanacaste World Heritage Site. It is a National Park in the northwestern part of Costa Rica which encompasses the Rincin de la Vieja and Santa Maria volcanoes, as well as the dormant Cerro Von Seebach.</obo:IAO_0000115>
        <oboInOwl:hasOBONamespace>GAZ</oboInOwl:hasOBONamespace>
        <oboInOwl:id>GAZ:00068700</oboInOwl:id>
        <rdfs:label>Parque Nacional Volcan Rincon de la Vieja</rdfs:label>
    </owl:NamedIndividual>
    


    <!-- http://purl.obolibrary.org/obo/GAZ_00068701 -->

    <owl:NamedIndividual rdf:about="http://purl.obolibrary.org/obo/GAZ_00068701">
        <obo:RO_0001025 rdf:resource="http://purl.obolibrary.org/obo/GAZ_00003206"/>
        <oboInOwl:hasOBONamespace>GAZ</oboInOwl:hasOBONamespace>
        <oboInOwl:id>GAZ:00068701</oboInOwl:id>
        <rdfs:label>Guacimo Canton</rdfs:label>
    </owl:NamedIndividual>
    


    <!-- http://purl.obolibrary.org/obo/GAZ_00068702 -->

    <owl:NamedIndividual rdf:about="http://purl.obolibrary.org/obo/GAZ_00068702">
        <obo:RO_0001025 rdf:resource="http://purl.obolibrary.org/obo/GAZ_00003208"/>
        <obo:IAO_0000115>The second canton in the province of Heredia in Costa Rica. The canton covers an area of 53.80 km2, The capital city of the canton is also called Barva. The elongated canton climbs from the city of Barva on the outskirts of the capital city of Heredia up the slopes of the dormant Barva Volcano, with the mountain&apos;s summit serving as its northern boundary.</obo:IAO_0000115>
        <oboInOwl:hasOBONamespace>GAZ</oboInOwl:hasOBONamespace>
        <oboInOwl:id>GAZ:00068702</oboInOwl:id>
        <rdfs:label>Barva Canton</rdfs:label>
    </owl:NamedIndividual>
    


    <!-- http://purl.obolibrary.org/obo/GAZ_00068703 -->

    <owl:NamedIndividual rdf:about="http://purl.obolibrary.org/obo/GAZ_00068703">
        <obo:RO_0001025 rdf:resource="http://purl.obolibrary.org/obo/GAZ_00003208"/>
        <obo:IAO_0000115>The first canton in the province of Heredia in Costa Rica. The canton covers an area of 282.60 km2. Its capital is the provincial capital city of Heredia, also known as Heredia Centro. The canton includes the areas south and west of the capital city of Heredia as far as the Rio Virilla and the General Canas Freeway (Autopista General Canas). The non-contiguous district of Varablanca, that includes a large portion of Braulio Carrillo National Park high in the Cordillera Central, is also administered as part of Heredia Canton.</obo:IAO_0000115>
        <oboInOwl:hasOBONamespace>GAZ</oboInOwl:hasOBONamespace>
        <oboInOwl:id>GAZ:00068703</oboInOwl:id>
        <rdfs:label>Heredia Canton</rdfs:label>
    </owl:NamedIndividual>
    


    <!-- http://purl.obolibrary.org/obo/GAZ_00068704 -->

    <owl:NamedIndividual rdf:about="http://purl.obolibrary.org/obo/GAZ_00068704">
        <obo:RO_0001025 rdf:resource="http://purl.obolibrary.org/obo/GAZ_00003208"/>
        <obo:IAO_0000115>The eighth canton in the province of Heredia in Costa Rica. The canton covers an area of 6.96 km2. The capital city of the canton is San Joaquin. The compact canton is located between the provincial capital cities of Alajuela and Heredia, with the Rio Segundo forming the northwestern boundary and the Rio Burio establishing the canton&apos;s southwestern border.</obo:IAO_0000115>
        <oboInOwl:hasOBONamespace>GAZ</oboInOwl:hasOBONamespace>
        <oboInOwl:id>GAZ:00068704</oboInOwl:id>
        <rdfs:label>Flores Canton</rdfs:label>
    </owl:NamedIndividual>
    


    <!-- http://purl.obolibrary.org/obo/GAZ_00068705 -->

    <owl:NamedIndividual rdf:about="http://purl.obolibrary.org/obo/GAZ_00068705">
        <obo:RO_0001025 rdf:resource="http://purl.obolibrary.org/obo/GAZ_00003208"/>
        <obo:IAO_0000115>The fifth canton in the province of Heredia in Costa Rica. The canton covers an area of 48.39 km2. The capital city of the canton is also called San Rafael. The canton is northeast of the provincial capital city of Heredia, reaching from the suburbs high into the Cordillera Central.</obo:IAO_0000115>
        <oboInOwl:hasOBONamespace>GAZ</oboInOwl:hasOBONamespace>
        <oboInOwl:id>GAZ:00068705</oboInOwl:id>
        <rdfs:label>San Rafael Canton</rdfs:label>
    </owl:NamedIndividual>
    


    <!-- http://purl.obolibrary.org/obo/GAZ_00068706 -->

    <owl:NamedIndividual rdf:about="http://purl.obolibrary.org/obo/GAZ_00068706">
        <obo:RO_0001025 rdf:resource="http://purl.obolibrary.org/obo/GAZ_00003208"/>
        <obo:IAO_0000115>The fourth canton in the province of Heredia in Costa Rica. The canton covers an area of 53.21 km2. The capital city of the canton is also called Santa Barbara. The elongated canton begins midway between the cities of Alajuela and Heredia, where the Rio Segundo marks its southern boundary. It climbs through foothills northward to the Rio Desengano high in the Cordillera Central.</obo:IAO_0000115>
        <oboInOwl:hasOBONamespace>GAZ</oboInOwl:hasOBONamespace>
        <oboInOwl:id>GAZ:00068706</oboInOwl:id>
        <rdfs:label>Santa Barbara Canton</rdfs:label>
    </owl:NamedIndividual>
    


    <!-- http://purl.obolibrary.org/obo/GAZ_00068707 -->

    <owl:NamedIndividual rdf:about="http://purl.obolibrary.org/obo/GAZ_00068707">
        <obo:RO_0001025 rdf:resource="http://purl.obolibrary.org/obo/GAZ_00003208"/>
        <obo:IAO_0000115>The third canton in the province of Heredia in Costa Rica. The canton covers an area of 24.84 km2, The capital city of the canton is also called Santo Domingo. The Rio Virilla on the south and the Rio Bermudez on the north establish the boundaries of this elongated province, which then climb up into the Cordillera Central with the Rio Para Blanca.</obo:IAO_0000115>
        <oboInOwl:hasOBONamespace>GAZ</oboInOwl:hasOBONamespace>
        <oboInOwl:id>GAZ:00068707</oboInOwl:id>
        <rdfs:label>Santo Domingo Canton</rdfs:label>
    </owl:NamedIndividual>
    


    <!-- http://purl.obolibrary.org/obo/GAZ_00068708 -->

    <owl:NamedIndividual rdf:about="http://purl.obolibrary.org/obo/GAZ_00068708">
        <obo:RO_0001025 rdf:resource="http://purl.obolibrary.org/obo/GAZ_00003208"/>
        <obo:IAO_0000115>The ninth canton in the province of Heredia in Costa Rica. The canton covers an area of 7.53 km2. The capital city of the canton is also called San Pablo. The canton is in the foothills southeast of the provincial capital city of Heredia, with the Rio Bermudez as the southeast boundary and the Rio Pirro delineating the farthest portion of the northwestern border. The canton of San Pablo is one of only two cantons in Costa Rica that is not subdivided into distritos (districts).</obo:IAO_0000115>
        <oboInOwl:hasOBONamespace>GAZ</oboInOwl:hasOBONamespace>
        <oboInOwl:id>GAZ:00068708</oboInOwl:id>
        <rdfs:label>San Pablo Canton</rdfs:label>
    </owl:NamedIndividual>
    


    <!-- http://purl.obolibrary.org/obo/GAZ_00068709 -->

    <owl:NamedIndividual rdf:about="http://purl.obolibrary.org/obo/GAZ_00068709">
        <obo:RO_0001025 rdf:resource="http://purl.obolibrary.org/obo/GAZ_00068702"/>
        <obo:RO_0001025 rdf:resource="http://purl.obolibrary.org/obo/GAZ_00068703"/>
        <obo:RO_0001025 rdf:resource="http://purl.obolibrary.org/obo/GAZ_00068773"/>
        <obo:RO_0001025 rdf:resource="http://purl.obolibrary.org/obo/GAZ_00068897"/>
        <obo:IAO_0000115>A national park of the Volcanic Cordillera Conservation Area in Costa Rica located on the eastern edge of the central volcanic corridor between San Jose and Puerto Limon.</obo:IAO_0000115>
        <oboInOwl:hasOBONamespace>GAZ</oboInOwl:hasOBONamespace>
        <oboInOwl:id>GAZ:00068709</oboInOwl:id>
        <rdfs:label>Braulio Carrillo National Park</rdfs:label>
    </owl:NamedIndividual>
    


    <!-- http://purl.obolibrary.org/obo/GAZ_00068711 -->

    <owl:NamedIndividual rdf:about="http://purl.obolibrary.org/obo/GAZ_00068711">
        <obo:RO_0001025 rdf:resource="http://purl.obolibrary.org/obo/GAZ_00056225"/>
        <obo:IAO_0000115>A crater lake.</obo:IAO_0000115>
        <oboInOwl:hasOBONamespace>GAZ</oboInOwl:hasOBONamespace>
        <oboInOwl:id>GAZ:00068711</oboInOwl:id>
        <rdfs:label>Danta Lake</rdfs:label>
    </owl:NamedIndividual>
    


    <!-- http://purl.obolibrary.org/obo/GAZ_00068712 -->

    <owl:NamedIndividual rdf:about="http://purl.obolibrary.org/obo/GAZ_00068712">
        <obo:RO_0001025 rdf:resource="http://purl.obolibrary.org/obo/GAZ_00056225"/>
        <obo:IAO_0000115>A crater lake.</obo:IAO_0000115>
        <oboInOwl:hasOBONamespace>GAZ</oboInOwl:hasOBONamespace>
        <oboInOwl:id>GAZ:00068712</oboInOwl:id>
        <rdfs:label>Barva Lake</rdfs:label>
    </owl:NamedIndividual>
    


    <!-- http://purl.obolibrary.org/obo/GAZ_00068713 -->

    <owl:NamedIndividual rdf:about="http://purl.obolibrary.org/obo/GAZ_00068713">
        <obo:RO_0001025 rdf:resource="http://purl.obolibrary.org/obo/GAZ_00056225"/>
        <obo:IAO_0000115>A crater lake.</obo:IAO_0000115>
        <oboInOwl:hasOBONamespace>GAZ</oboInOwl:hasOBONamespace>
        <oboInOwl:id>GAZ:00068713</oboInOwl:id>
        <rdfs:label>Copey Lake</rdfs:label>
    </owl:NamedIndividual>
    


    <!-- http://purl.obolibrary.org/obo/GAZ_00068714 -->

    <owl:NamedIndividual rdf:about="http://purl.obolibrary.org/obo/GAZ_00068714">
        <rdf:type rdf:resource="http://purl.obolibrary.org/obo/ENVO_00000004"/>
        <obo:RO_0001025 rdf:resource="http://purl.obolibrary.org/obo/GAZ_00009458"/>
        <obo:IAO_0000115>A district of San Isidro Canton.</obo:IAO_0000115>
        <oboInOwl:hasOBONamespace>GAZ</oboInOwl:hasOBONamespace>
        <oboInOwl:id>GAZ:00068714</oboInOwl:id>
        <rdfs:label>San Isidro District</rdfs:label>
    </owl:NamedIndividual>
    


    <!-- http://purl.obolibrary.org/obo/GAZ_00068715 -->

    <owl:NamedIndividual rdf:about="http://purl.obolibrary.org/obo/GAZ_00068715">
        <rdf:type rdf:resource="http://purl.obolibrary.org/obo/ENVO_00000004"/>
        <obo:RO_0001025 rdf:resource="http://purl.obolibrary.org/obo/GAZ_00009458"/>
        <obo:IAO_0000115>A district of San Isidro Canton.</obo:IAO_0000115>
        <oboInOwl:hasOBONamespace>GAZ</oboInOwl:hasOBONamespace>
        <oboInOwl:id>GAZ:00068715</oboInOwl:id>
        <rdfs:label>San Francisco District</rdfs:label>
    </owl:NamedIndividual>
    


    <!-- http://purl.obolibrary.org/obo/GAZ_00068716 -->

    <owl:NamedIndividual rdf:about="http://purl.obolibrary.org/obo/GAZ_00068716">
        <rdf:type rdf:resource="http://purl.obolibrary.org/obo/ENVO_00000004"/>
        <obo:RO_0001025 rdf:resource="http://purl.obolibrary.org/obo/GAZ_00009458"/>
        <obo:IAO_0000115>A district of San Isidro Canton.</obo:IAO_0000115>
        <oboInOwl:hasOBONamespace>GAZ</oboInOwl:hasOBONamespace>
        <oboInOwl:id>GAZ:00068716</oboInOwl:id>
        <rdfs:label>Concepcion District</rdfs:label>
    </owl:NamedIndividual>
    


    <!-- http://purl.obolibrary.org/obo/GAZ_00068717 -->

    <owl:NamedIndividual rdf:about="http://purl.obolibrary.org/obo/GAZ_00068717">
        <rdf:type rdf:resource="http://purl.obolibrary.org/obo/ENVO_00000004"/>
        <obo:RO_0001025 rdf:resource="http://purl.obolibrary.org/obo/GAZ_00009458"/>
        <obo:IAO_0000115>A district of San Isidro Canton.</obo:IAO_0000115>
        <oboInOwl:hasOBONamespace>GAZ</oboInOwl:hasOBONamespace>
        <oboInOwl:id>GAZ:00068717</oboInOwl:id>
        <rdfs:label>San Jose District</rdfs:label>
    </owl:NamedIndividual>
    


    <!-- http://purl.obolibrary.org/obo/GAZ_00068718 -->

    <owl:NamedIndividual rdf:about="http://purl.obolibrary.org/obo/GAZ_00068718">
        <obo:RO_0001025 rdf:resource="http://purl.obolibrary.org/obo/GAZ_00003206"/>
        <oboInOwl:hasOBONamespace>GAZ</oboInOwl:hasOBONamespace>
        <oboInOwl:id>GAZ:00068718</oboInOwl:id>
        <rdfs:label>Matina Canton</rdfs:label>
    </owl:NamedIndividual>
    


    <!-- http://purl.obolibrary.org/obo/GAZ_00068719 -->

    <owl:NamedIndividual rdf:about="http://purl.obolibrary.org/obo/GAZ_00068719">
        <obo:RO_0001025 rdf:resource="http://purl.obolibrary.org/obo/GAZ_00003206"/>
        <obo:IAO_0000115>A canton in the central region of the province of Limon. Its capital is Siquirres.</obo:IAO_0000115>
        <oboInOwl:hasOBONamespace>GAZ</oboInOwl:hasOBONamespace>
        <oboInOwl:id>GAZ:00068719</oboInOwl:id>
        <rdfs:label>Siquirres Canton</rdfs:label>
    </owl:NamedIndividual>
    


    <!-- http://purl.obolibrary.org/obo/GAZ_00068720 -->

    <owl:NamedIndividual rdf:about="http://purl.obolibrary.org/obo/GAZ_00068720">
        <obo:RO_0001025 rdf:resource="http://purl.obolibrary.org/obo/GAZ_00003206"/>
        <oboInOwl:hasOBONamespace>GAZ</oboInOwl:hasOBONamespace>
        <oboInOwl:id>GAZ:00068720</oboInOwl:id>
        <rdfs:label>Limon Canton</rdfs:label>
    </owl:NamedIndividual>
    


    <!-- http://purl.obolibrary.org/obo/GAZ_00068721 -->

    <owl:NamedIndividual rdf:about="http://purl.obolibrary.org/obo/GAZ_00068721">
        <obo:RO_0001025 rdf:resource="http://purl.obolibrary.org/obo/GAZ_00003206"/>
        <obo:IAO_0000115>The fourth canton in the province of Limon in Costa Rica. The canton covers an area of 576.48 km2 Its capital city is also called Guacimo. The canton includes all of the Caribbean coast south of Rio Tuba. It shares its eastern border with Panama, and encompasses a major portion of the Cordillera de Talamanca and the indigenous reserves in the area.</obo:IAO_0000115>
        <oboInOwl:hasOBONamespace>GAZ</oboInOwl:hasOBONamespace>
        <oboInOwl:id>GAZ:00068721</oboInOwl:id>
        <rdfs:label>Talamanca Canton</rdfs:label>
    </owl:NamedIndividual>
    


    <!-- http://purl.obolibrary.org/obo/GAZ_00068722 -->

    <owl:NamedIndividual rdf:about="http://purl.obolibrary.org/obo/GAZ_00068722">
        <obo:RO_0001025 rdf:resource="http://purl.obolibrary.org/obo/GAZ_00003206"/>
        <obo:IAO_0000115>The second canton in the province of Limon in Costa Rica. The canton covers an area of 2,403.49 km2. Its capital in the city of Guapiles The canton takes in the Caribbean coast from the Rio Toro northward to the border with Nicaragua. It ranges inland in a southwestern direction with the Rio Chirripo forming the western border. The canton ends in the Cordillera Central where the Rio Sucio crosses the highway in Braulio Carrillo National Park.</obo:IAO_0000115>
        <oboInOwl:hasOBONamespace>GAZ</oboInOwl:hasOBONamespace>
        <oboInOwl:id>GAZ:00068722</oboInOwl:id>
        <rdfs:label>Pococi Canton</rdfs:label>
    </owl:NamedIndividual>
    


    <!-- http://purl.obolibrary.org/obo/GAZ_00068723 -->

    <owl:NamedIndividual rdf:about="http://purl.obolibrary.org/obo/GAZ_00068723">
        <obo:RO_0001025 rdf:resource="http://purl.obolibrary.org/obo/GAZ_00068722"/>
        <obo:RO_0001025 rdf:resource="http://purl.obolibrary.org/obo/GAZ_00068836"/>
        <obo:IAO_0000115>A national park within the Tortuguero Conservation Area. The reserve is also included in the Humedal Caribe Noreste, a wetland of international importance under the Ramsar Convention. The park is located in the Limon Province of northeastern Costa Rica.</obo:IAO_0000115>
        <oboInOwl:hasOBONamespace>GAZ</oboInOwl:hasOBONamespace>
        <oboInOwl:id>GAZ:00068723</oboInOwl:id>
        <rdfs:label>Tortuguero National Park</rdfs:label>
    </owl:NamedIndividual>
    


    <!-- http://purl.obolibrary.org/obo/GAZ_00068724 -->

    <owl:NamedIndividual rdf:about="http://purl.obolibrary.org/obo/GAZ_00068724">
        <obo:RO_0001025 rdf:resource="http://purl.obolibrary.org/obo/GAZ_00003206"/>
        <obo:RO_0001025 rdf:resource="http://purl.obolibrary.org/obo/GAZ_00068836"/>
        <obo:IAO_0000115>A wildlife refuge located within the Tortuguero Conservation Area, in the Limnn Province of northeastern Costa Rica. The refuge is located north of the village of Tortuguero, between the Barra del Colorado Wildlife Refuge and the Tortuguero National Park.</obo:IAO_0000115>
        <oboInOwl:hasOBONamespace>GAZ</oboInOwl:hasOBONamespace>
        <oboInOwl:id>GAZ:00068724</oboInOwl:id>
        <rdfs:label>Dr. Archie Carr Wildlife Refuge</rdfs:label>
    </owl:NamedIndividual>
    


    <!-- http://purl.obolibrary.org/obo/GAZ_00068725 -->

    <owl:NamedIndividual rdf:about="http://purl.obolibrary.org/obo/GAZ_00068725">
        <obo:RO_0001025 rdf:resource="http://purl.obolibrary.org/obo/GAZ_00068722"/>
        <obo:RO_0001025 rdf:resource="http://purl.obolibrary.org/obo/GAZ_00068836"/>
        <obo:IAO_0000115>A wildlife refuge, part of the Tortuguero Conservation Area, in Limon Province in the northeastern part of Costa Rica.</obo:IAO_0000115>
        <oboInOwl:hasOBONamespace>GAZ</oboInOwl:hasOBONamespace>
        <oboInOwl:id>GAZ:00068725</oboInOwl:id>
        <rdfs:label>Barra del Colorado Wildlife Refuge</rdfs:label>
    </owl:NamedIndividual>
    


    <!-- http://purl.obolibrary.org/obo/GAZ_00068726 -->

    <owl:NamedIndividual rdf:about="http://purl.obolibrary.org/obo/GAZ_00068726">
        <obo:RO_0001025 rdf:resource="http://purl.obolibrary.org/obo/GAZ_00003209"/>
        <obo:RO_0001025 rdf:resource="http://purl.obolibrary.org/obo/GAZ_00068734"/>
        <obo:RO_0001025 rdf:resource="http://purl.obolibrary.org/obo/GAZ_00068735"/>
        <obo:IAO_0000115>A small National Park in the Central Pacific Conservation Area located on the Pacific coast of Costa Rica, just south of the city of Quepos, Puntarenas, and 132 km from the national capital of San Jose. Established in 1972.</obo:IAO_0000115>
        <oboInOwl:hasOBONamespace>GAZ</oboInOwl:hasOBONamespace>
        <oboInOwl:id>GAZ:00068726</oboInOwl:id>
        <rdfs:label>Parque Nacional Manuel Antonio</rdfs:label>
    </owl:NamedIndividual>
    


    <!-- http://purl.obolibrary.org/obo/GAZ_00068727 -->

    <owl:NamedIndividual rdf:about="http://purl.obolibrary.org/obo/GAZ_00068727">
        <obo:RO_0001025 rdf:resource="http://purl.obolibrary.org/obo/GAZ_00003209"/>
        <obo:IAO_0000115>The fifth canton in the province of Puntarenas in Costa Rica. The canton covers an area of 1,930.24 km2. Its capital city is Ciudad Cortes, formerly known as Puerto Cortes. The canton begins at the Rio Baru near Dominical on the central Pacific coast. It continues as a narrow strip of land southward to include the area around Palmar and Sierpe, finally widening to take in the entire neck and upper portion of the Osa Peninsula.</obo:IAO_0000115>
        <oboInOwl:hasOBONamespace>GAZ</oboInOwl:hasOBONamespace>
        <oboInOwl:id>GAZ:00068727</oboInOwl:id>
        <rdfs:label>Osa Canton</rdfs:label>
    </owl:NamedIndividual>
    


    <!-- http://purl.obolibrary.org/obo/GAZ_00068728 -->

    <owl:NamedIndividual rdf:about="http://purl.obolibrary.org/obo/GAZ_00068728">
        <obo:RO_0001025 rdf:resource="http://purl.obolibrary.org/obo/GAZ_00003209"/>
        <obo:IAO_0000115>The tenth canton in the province of Puntarenas in Costa Rica. The canton covers an area of 620.60 km2. Its capital city is Ciudad Neily. The lowland canton shares its eastern border with Panama. The Rio Conte marks the western limit. The northern boundary runs through the Fila Zapote, one of the coastal mountain ranges.</obo:IAO_0000115>
        <oboInOwl:hasOBONamespace>GAZ</oboInOwl:hasOBONamespace>
        <oboInOwl:id>GAZ:00068728</oboInOwl:id>
        <rdfs:label>Corredores Canton</rdfs:label>
    </owl:NamedIndividual>
    


    <!-- http://purl.obolibrary.org/obo/GAZ_00068729 -->

    <owl:NamedIndividual rdf:about="http://purl.obolibrary.org/obo/GAZ_00068729">
        <obo:RO_0001025 rdf:resource="http://purl.obolibrary.org/obo/GAZ_00003209"/>
        <obo:IAO_0000115>The third canton in the province of Puntarenas in Costa Rica. The canton covers an area of 2,384.22 km2. Its capital city is also called Buenos Aires. The canton includes a portion of the Cordillera de Talamaca along its northeastern border. The valleys of the Rio General, Rio Coto Brus and Rio Terraba form the core of the canton, and coastal mountain ranges set the limits on the southeast side.</obo:IAO_0000115>
        <oboInOwl:hasOBONamespace>GAZ</oboInOwl:hasOBONamespace>
        <oboInOwl:id>GAZ:00068729</oboInOwl:id>
        <rdfs:label>Buenos Aires Canton</rdfs:label>
    </owl:NamedIndividual>
    


    <!-- http://purl.obolibrary.org/obo/GAZ_00068730 -->

    <owl:NamedIndividual rdf:about="http://purl.obolibrary.org/obo/GAZ_00068730">
        <obo:RO_0001025 rdf:resource="http://purl.obolibrary.org/obo/GAZ_00003209"/>
        <obo:IAO_0000115>The eleventh canton in the province of Puntarenas in Costa Rica. The canton covers an area of 316.31 km2. Its capital city is Jaco. The canton lies along the north-central Pacific coast between Punta Loros near the town of Tivives and the mouth of the Rio Tusubres. The eastern boundary runs through the Fila Negra, a coastal mountain range.</obo:IAO_0000115>
        <oboInOwl:hasOBONamespace>GAZ</oboInOwl:hasOBONamespace>
        <oboInOwl:id>GAZ:00068730</oboInOwl:id>
        <rdfs:label>Garabito Canton</rdfs:label>
    </owl:NamedIndividual>
    


    <!-- http://purl.obolibrary.org/obo/GAZ_00068731 -->

    <owl:NamedIndividual rdf:about="http://purl.obolibrary.org/obo/GAZ_00068731">
        <obo:RO_0001025 rdf:resource="http://purl.obolibrary.org/obo/GAZ_00003209"/>
        <obo:IAO_0000115>The second canton in the province of Puntarenas in Costa Rica. The canton covers an area of 216.80 km2. Its capital city is also called Esparza. The major portion of the canton lies along the coast of the Gulf of Nicoya between the mouths of Rio Barranca and the Rio Jesus Maria. An extension of the canton reaches northward from Esparza into the Cordillera de Tilaran.</obo:IAO_0000115>
        <oboInOwl:hasOBONamespace>GAZ</oboInOwl:hasOBONamespace>
        <oboInOwl:id>GAZ:00068731</oboInOwl:id>
        <rdfs:label>Esparza Canton</rdfs:label>
    </owl:NamedIndividual>
    


    <!-- http://purl.obolibrary.org/obo/GAZ_00068732 -->

    <owl:NamedIndividual rdf:about="http://purl.obolibrary.org/obo/GAZ_00068732">
        <obo:RO_0001025 rdf:resource="http://purl.obolibrary.org/obo/GAZ_00003209"/>
        <obo:IAO_0000115>The fourth canton in the province of Puntarenas in Costa Rica. The canton covers an area of 208.34 km2. Its capital city is Miramar. The mountainous canton lies in the Cordillera de Tilaran northeast of the city of Puntarenas. It is limited on the north by the Rio Aranjuez. The Rio San Miguel and Rio Tiacinto delineate the southern boundary.</obo:IAO_0000115>
        <oboInOwl:hasOBONamespace>GAZ</oboInOwl:hasOBONamespace>
        <oboInOwl:id>GAZ:00068732</oboInOwl:id>
        <rdfs:label>Montes de Oro Canton</rdfs:label>
    </owl:NamedIndividual>
    


    <!-- http://purl.obolibrary.org/obo/GAZ_00068733 -->

    <owl:NamedIndividual rdf:about="http://purl.obolibrary.org/obo/GAZ_00068733">
        <obo:RO_0001025 rdf:resource="http://purl.obolibrary.org/obo/GAZ_00003209"/>
        <obo:IAO_0000115>The name of the ninth canton in the province of Puntarenas in Costa Rica. The canton covers an area of 478.79 km2. Its capital city is also called Parrita. The canton lies along the central Pacific coast between the mouths of the Rio Tusubres and iio Damas. Inland the canton is delineated by a series of rivers that meander through the valleys of the coastal mountain range. The canton of Parrita is one of only two cantons in Costa Rica that is not subdivided into distritos (districts).</obo:IAO_0000115>
        <oboInOwl:hasOBONamespace>GAZ</oboInOwl:hasOBONamespace>
        <oboInOwl:id>GAZ:00068733</oboInOwl:id>
        <rdfs:label>Parrita Canton</rdfs:label>
    </owl:NamedIndividual>
    


    <!-- http://purl.obolibrary.org/obo/GAZ_00068734 -->

    <owl:NamedIndividual rdf:about="http://purl.obolibrary.org/obo/GAZ_00068734">
        <obo:RO_0001025 rdf:resource="http://purl.obolibrary.org/obo/GAZ_00003209"/>
        <obo:IAO_0000115>The sixth canton in the province of Puntarenas in Costa Rica. The canton covers an area of 543.77 km2. Its capital city is Quepos, also known as Puerto Quepos. The canton lies along the central Pacific coast between the mouths of the Rio Damas and Rio Baru. The northeastern border runs through high, remote coastal mountain ranges.</obo:IAO_0000115>
        <oboInOwl:hasOBONamespace>GAZ</oboInOwl:hasOBONamespace>
        <oboInOwl:id>GAZ:00068734</oboInOwl:id>
        <rdfs:label>Aguirre Canton</rdfs:label>
    </owl:NamedIndividual>
    


    <!-- http://purl.obolibrary.org/obo/GAZ_00068735 -->

    <owl:NamedIndividual rdf:about="http://purl.obolibrary.org/obo/GAZ_00068735">
        <obo:RO_0001025 rdf:resource="http://purl.obolibrary.org/obo/GAZ_00002901"/>
        <obo:IAO_0000115>An administrative area which is managed by the Sistema Nacional de Areas de Conservacion for the purposes of conservation in the southwestern part of Costa Rica, on the Pacific coast. It contains three National Parks, and a number Wildlife refuges and other types of nature reserve.</obo:IAO_0000115>
        <oboInOwl:hasOBONamespace>GAZ</oboInOwl:hasOBONamespace>
        <oboInOwl:id>GAZ:00068735</oboInOwl:id>
        <rdfs:label>Central Pacific Conservation Area</rdfs:label>
    </owl:NamedIndividual>
    


    <!-- http://purl.obolibrary.org/obo/GAZ_00068736 -->

    <owl:NamedIndividual rdf:about="http://purl.obolibrary.org/obo/GAZ_00068736">
        <obo:RO_0001025 rdf:resource="http://purl.obolibrary.org/obo/GAZ_00003209"/>
        <obo:IAO_0000115>An inlet in Costa Rica. The inlet starts on the Pacific Ocean side of Costa Rica and extends slightly northward before turning west. The most westward part is at the city of Rincon. The bay separates the Osa Peninsula from the mainland Costa Rica.</obo:IAO_0000115>
        <oboInOwl:hasOBONamespace>GAZ</oboInOwl:hasOBONamespace>
        <oboInOwl:id>GAZ:00068736</oboInOwl:id>
        <rdfs:label>Gulf of Dulce</rdfs:label>
    </owl:NamedIndividual>
    


    <!-- http://purl.obolibrary.org/obo/GAZ_00068737 -->

    <owl:NamedIndividual rdf:about="http://purl.obolibrary.org/obo/GAZ_00068737">
        <obo:RO_0001025 rdf:resource="http://purl.obolibrary.org/obo/GAZ_00068738"/>
        <obo:IAO_0000115>A peninsula located in southwestern Costa Rica, in the Puntarenas Province, on the Pacific Ocean.</obo:IAO_0000115>
        <oboInOwl:hasOBONamespace>GAZ</oboInOwl:hasOBONamespace>
        <oboInOwl:id>GAZ:00068737</oboInOwl:id>
        <rdfs:label>Peninsula de Osa</rdfs:label>
    </owl:NamedIndividual>
    


    <!-- http://purl.obolibrary.org/obo/GAZ_00068738 -->

    <owl:NamedIndividual rdf:about="http://purl.obolibrary.org/obo/GAZ_00068738">
        <obo:RO_0001025 rdf:resource="http://purl.obolibrary.org/obo/GAZ_00003209"/>
        <obo:IAO_0000115>An administrative area which is managed by SINAC for the purposes of conservation in Costa Rica, on the southern Pacific coast region. It contains two National Parks, and numerous Wildlife refuges and other types of nature reserve.</obo:IAO_0000115>
        <oboInOwl:hasOBONamespace>GAZ</oboInOwl:hasOBONamespace>
        <oboInOwl:id>GAZ:00068738</oboInOwl:id>
        <rdfs:label>Osa Conservation Area</rdfs:label>
    </owl:NamedIndividual>
    


    <!-- http://purl.obolibrary.org/obo/GAZ_00068739 -->

    <owl:NamedIndividual rdf:about="http://purl.obolibrary.org/obo/GAZ_00068739">
        <obo:RO_0001025 rdf:resource="http://purl.obolibrary.org/obo/GAZ_00068737"/>
        <obo:IAO_0000115>A national park on the Osa Peninsula in the South West of Costa Rica which is part of the Osa Conservation Area. Established 1975-10-24.</obo:IAO_0000115>
        <oboInOwl:hasOBONamespace>GAZ</oboInOwl:hasOBONamespace>
        <oboInOwl:id>GAZ:00068739</oboInOwl:id>
        <rdfs:label>Parque Nacional Corcovado</rdfs:label>
    </owl:NamedIndividual>
    


    <!-- http://purl.obolibrary.org/obo/GAZ_00068740 -->

    <owl:NamedIndividual rdf:about="http://purl.obolibrary.org/obo/GAZ_00068740">
        <obo:RO_0001025 rdf:resource="http://purl.obolibrary.org/obo/GAZ_00068738"/>
        <obo:IAO_0000115>A national park part of the Osa Conservation Area it is found in the Puntarenas Province of southern Costa Rica near the town of La Gamba. It protects rainforests and beaches near the Golfo Dulce on the Pacific Coast.</obo:IAO_0000115>
        <oboInOwl:hasOBONamespace>GAZ</oboInOwl:hasOBONamespace>
        <oboInOwl:id>GAZ:00068740</oboInOwl:id>
        <rdfs:label>Piedras Blancas National Park</rdfs:label>
    </owl:NamedIndividual>
    


    <!-- http://purl.obolibrary.org/obo/GAZ_00068741 -->

    <owl:NamedIndividual rdf:about="http://purl.obolibrary.org/obo/GAZ_00068741">
        <obo:RO_0001025 rdf:resource="http://purl.obolibrary.org/obo/GAZ_00068738"/>
        <obo:IAO_0000115>An area that protects forested beach areas on the southern tip of the Osa Peninsula, Cabo Matapalo, Pacific Coast of Costa Rica.</obo:IAO_0000115>
        <oboInOwl:hasOBONamespace>GAZ</oboInOwl:hasOBONamespace>
        <oboInOwl:id>GAZ:00068741</oboInOwl:id>
        <rdfs:label>Osa Wildlife Refuge</rdfs:label>
    </owl:NamedIndividual>
    


    <!-- http://purl.obolibrary.org/obo/GAZ_00068742 -->

    <owl:NamedIndividual rdf:about="http://purl.obolibrary.org/obo/GAZ_00068742">
        <obo:RO_0001025 rdf:resource="http://purl.obolibrary.org/obo/GAZ_00068738"/>
        <obo:IAO_0000115>An area that protectsthe coral and rock reefs in Coronado Bay, south of Costa Rica.</obo:IAO_0000115>
        <oboInOwl:hasOBONamespace>GAZ</oboInOwl:hasOBONamespace>
        <oboInOwl:id>GAZ:00068742</oboInOwl:id>
        <rdfs:label>Ballena National Marine Park</rdfs:label>
    </owl:NamedIndividual>
    


    <!-- http://purl.obolibrary.org/obo/GAZ_00068743 -->

    <owl:NamedIndividual rdf:about="http://purl.obolibrary.org/obo/GAZ_00068743">
        <obo:RO_0001025 rdf:resource="http://purl.obolibrary.org/obo/GAZ_00068738"/>
        <obo:IAO_0000115>An area that protects forested and beach areas surrounding Golfito Costa Rica on the Golfo Dulce, Pacific Coast.</obo:IAO_0000115>
        <oboInOwl:hasOBONamespace>GAZ</oboInOwl:hasOBONamespace>
        <oboInOwl:id>GAZ:00068743</oboInOwl:id>
        <rdfs:label>Golfito Wildlife Refuge</rdfs:label>
    </owl:NamedIndividual>
    


    <!-- http://purl.obolibrary.org/obo/GAZ_00068744 -->

    <owl:NamedIndividual rdf:about="http://purl.obolibrary.org/obo/GAZ_00068744">
        <obo:RO_0001025 rdf:resource="http://purl.obolibrary.org/obo/GAZ_00068738"/>
        <obo:IAO_0000115>An area that Park Attractions The Donald Peters Hayes Wildlife Refuge protects forested areas near Golfito overlooking the Golfo Dulce, Pacific Coast of Costa Rica.</obo:IAO_0000115>
        <oboInOwl:hasOBONamespace>GAZ</oboInOwl:hasOBONamespace>
        <oboInOwl:id>GAZ:00068744</oboInOwl:id>
        <rdfs:label>Donald Peters Hayes Wildlife Refuge</rdfs:label>
    </owl:NamedIndividual>
    


    <!-- http://purl.obolibrary.org/obo/GAZ_00068745 -->

    <owl:NamedIndividual rdf:about="http://purl.obolibrary.org/obo/GAZ_00068745">
        <obo:RO_0001025 rdf:resource="http://purl.obolibrary.org/obo/GAZ_00068738"/>
        <obo:IAO_0000115>An area that protects forested and beach areas near Punta Uvita and Ballena National Marine Park, Pacific Coast of Costa Rica.</obo:IAO_0000115>
        <oboInOwl:hasOBONamespace>GAZ</oboInOwl:hasOBONamespace>
        <oboInOwl:id>GAZ:00068745</oboInOwl:id>
        <rdfs:label>Rancho La Merced Wildlife Refuge</rdfs:label>
    </owl:NamedIndividual>
    


    <!-- http://purl.obolibrary.org/obo/GAZ_00068746 -->

    <owl:NamedIndividual rdf:about="http://purl.obolibrary.org/obo/GAZ_00068746">
        <obo:RO_0001025 rdf:resource="http://purl.obolibrary.org/obo/GAZ_00068738"/>
        <obo:IAO_0000115>An area that protects forested and beach areas in the Drake Bay region of the Osa Peninsula, Pacific Coast of Costa Rica. 8 miles north of Corcovado National Park.</obo:IAO_0000115>
        <oboInOwl:hasOBONamespace>GAZ</oboInOwl:hasOBONamespace>
        <oboInOwl:id>GAZ:00068746</oboInOwl:id>
        <rdfs:label>Quillotro Wildlife Refuge</rdfs:label>
    </owl:NamedIndividual>
    


    <!-- http://purl.obolibrary.org/obo/GAZ_00068747 -->

    <owl:NamedIndividual rdf:about="http://purl.obolibrary.org/obo/GAZ_00068747">
        <obo:RO_0001025 rdf:resource="http://purl.obolibrary.org/obo/GAZ_00068738"/>
        <obo:IAO_0000115>A protected area.</obo:IAO_0000115>
        <oboInOwl:hasOBONamespace>GAZ</oboInOwl:hasOBONamespace>
        <oboInOwl:id>GAZ:00068747</oboInOwl:id>
        <rdfs:label>Golfo Dulce Forest Reserve</rdfs:label>
    </owl:NamedIndividual>
    


    <!-- http://purl.obolibrary.org/obo/GAZ_00068748 -->

    <owl:NamedIndividual rdf:about="http://purl.obolibrary.org/obo/GAZ_00068748">
        <obo:RO_0001025 rdf:resource="http://purl.obolibrary.org/obo/GAZ_00068738"/>
        <obo:IAO_0000115>An area that protects forested and beach areas on the Osa Peninsula and Golfo Dulce, Pacific Coast of Costa Rica.</obo:IAO_0000115>
        <oboInOwl:hasOBONamespace>GAZ</oboInOwl:hasOBONamespace>
        <oboInOwl:id>GAZ:00068748</oboInOwl:id>
        <rdfs:label>Preciosa Platanares Wildlife Refuge</rdfs:label>
    </owl:NamedIndividual>
    


    <!-- http://purl.obolibrary.org/obo/GAZ_00068749 -->

    <owl:NamedIndividual rdf:about="http://purl.obolibrary.org/obo/GAZ_00068749">
        <obo:RO_0001025 rdf:resource="http://purl.obolibrary.org/obo/GAZ_00068747"/>
        <obo:IAO_0000115>An area that protects forested river areas on the southern Osa Peninsula, Pacific Coast of Costa Rica. It lies entirely within the Golfo Dulce Forest Reserve, near Puerto Jimenez.</obo:IAO_0000115>
        <oboInOwl:hasOBONamespace>GAZ</oboInOwl:hasOBONamespace>
        <oboInOwl:id>GAZ:00068749</oboInOwl:id>
        <rdfs:label>Hacienda Copano Wildlife Refuge</rdfs:label>
    </owl:NamedIndividual>
    


    <!-- http://purl.obolibrary.org/obo/GAZ_00068750 -->

    <owl:NamedIndividual rdf:about="http://purl.obolibrary.org/obo/GAZ_00068750">
        <obo:RO_0001025 rdf:resource="http://purl.obolibrary.org/obo/GAZ_00068738"/>
        <obo:IAO_0000115>An area that protects lowland areas on the southern Osa Peninsula, Pacific Coast of Costa Rica.</obo:IAO_0000115>
        <oboInOwl:hasOBONamespace>GAZ</oboInOwl:hasOBONamespace>
        <oboInOwl:id>GAZ:00068750</oboInOwl:id>
        <rdfs:label>Pejeperro Wildlife Refuge</rdfs:label>
    </owl:NamedIndividual>
    


    <!-- http://purl.obolibrary.org/obo/GAZ_00068751 -->

    <owl:NamedIndividual rdf:about="http://purl.obolibrary.org/obo/GAZ_00068751">
        <obo:RO_0001025 rdf:resource="http://purl.obolibrary.org/obo/GAZ_00068738"/>
        <obo:IAO_0000115>An area that protects forested and beach areas on the Osa Peninsula, Pacific Coast of Costa Rica.</obo:IAO_0000115>
        <oboInOwl:hasOBONamespace>GAZ</oboInOwl:hasOBONamespace>
        <oboInOwl:id>GAZ:00068751</oboInOwl:id>
        <rdfs:label>Carate Wildlife Refuge</rdfs:label>
    </owl:NamedIndividual>
    


    <!-- http://purl.obolibrary.org/obo/GAZ_00068752 -->

    <owl:NamedIndividual rdf:about="http://purl.obolibrary.org/obo/GAZ_00068752">
        <obo:RO_0001025 rdf:resource="http://purl.obolibrary.org/obo/GAZ_00068738"/>
        <obo:IAO_0000115>An area that protects forested and beach areas in the Drake Bay area of the Osa Peninsula, Pacific Coast of Costa Rica.</obo:IAO_0000115>
        <oboInOwl:hasOBONamespace>GAZ</oboInOwl:hasOBONamespace>
        <oboInOwl:id>GAZ:00068752</oboInOwl:id>
        <rdfs:label>Punta Rio Claro Wildlife Refuge</rdfs:label>
    </owl:NamedIndividual>
    


    <!-- http://purl.obolibrary.org/obo/GAZ_00068753 -->

    <owl:NamedIndividual rdf:about="http://purl.obolibrary.org/obo/GAZ_00068753">
        <obo:RO_0001025 rdf:resource="http://purl.obolibrary.org/obo/GAZ_00068738"/>
        <obo:IAO_0000115>An area that protects forested rural areas inland of the Golfo Dulce, Pacific Coast of Costa Rica.</obo:IAO_0000115>
        <oboInOwl:hasOBONamespace>GAZ</oboInOwl:hasOBONamespace>
        <oboInOwl:id>GAZ:00068753</oboInOwl:id>
        <rdfs:label>Agua Buena Wildlife Refuge</rdfs:label>
    </owl:NamedIndividual>
    


    <!-- http://purl.obolibrary.org/obo/GAZ_00068754 -->

    <owl:NamedIndividual rdf:about="http://purl.obolibrary.org/obo/GAZ_00068754">
        <obo:RO_0001025 rdf:resource="http://purl.obolibrary.org/obo/GAZ_00068738"/>
        <obo:IAO_0000115>An area that protects the extensive river mouth delta systems, estuaries and wetlands between the Terraba River and the Sierpe River on the Pacific Coast of Costa Rica, north of Drake Bay.</obo:IAO_0000115>
        <oboInOwl:hasOBONamespace>GAZ</oboInOwl:hasOBONamespace>
        <oboInOwl:id>GAZ:00068754</oboInOwl:id>
        <rdfs:label>Terraba-Sierpe National Wetlands</rdfs:label>
    </owl:NamedIndividual>
    


    <!-- http://purl.obolibrary.org/obo/GAZ_00068755 -->

    <owl:NamedIndividual rdf:about="http://purl.obolibrary.org/obo/GAZ_00068755">
        <obo:RO_0001025 rdf:resource="http://purl.obolibrary.org/obo/GAZ_00068738"/>
        <obo:IAO_0000115>A protected area.</obo:IAO_0000115>
        <oboInOwl:hasOBONamespace>GAZ</oboInOwl:hasOBONamespace>
        <oboInOwl:id>GAZ:00068755</oboInOwl:id>
        <rdfs:label>Cano Island Biological Reserve</rdfs:label>
    </owl:NamedIndividual>
    


    <!-- http://purl.obolibrary.org/obo/GAZ_00068756 -->

    <owl:NamedIndividual rdf:about="http://purl.obolibrary.org/obo/GAZ_00068756">
        <obo:RO_0001025 rdf:resource="http://purl.obolibrary.org/obo/GAZ_00068738"/>
        <obo:IAO_0000115>An area that protects mouth of the Rio Oro and beach areas on the southern Osa Peninsula, Pacific Coast of Costa Rica.</obo:IAO_0000115>
        <oboInOwl:hasOBONamespace>GAZ</oboInOwl:hasOBONamespace>
        <oboInOwl:id>GAZ:00068756</oboInOwl:id>
        <rdfs:label>Rio Oro Wildlife Refuge</rdfs:label>
    </owl:NamedIndividual>
    


    <!-- http://purl.obolibrary.org/obo/GAZ_00068757 -->

    <owl:NamedIndividual rdf:about="http://purl.obolibrary.org/obo/GAZ_00068757">
        <obo:RO_0001025 rdf:resource="http://purl.obolibrary.org/obo/GAZ_00068738"/>
        <obo:IAO_0000115>An area that protects forested and beach areas on the Osa Peninsula, Pacific Coast of Costa Rica.</obo:IAO_0000115>
        <oboInOwl:hasOBONamespace>GAZ</oboInOwl:hasOBONamespace>
        <oboInOwl:id>GAZ:00068757</oboInOwl:id>
        <rdfs:label>Lagunazul Wildlife Refuge</rdfs:label>
    </owl:NamedIndividual>
    


    <!-- http://purl.obolibrary.org/obo/GAZ_00068758 -->

    <owl:NamedIndividual rdf:about="http://purl.obolibrary.org/obo/GAZ_00068758">
        <obo:RO_0001025 rdf:resource="http://purl.obolibrary.org/obo/GAZ_00068738"/>
        <obo:IAO_0000115>An area that protects lowland areas on the southern Osa Peninsula, Pacific Coast of Costa Rica.</obo:IAO_0000115>
        <oboInOwl:hasOBONamespace>GAZ</oboInOwl:hasOBONamespace>
        <oboInOwl:id>GAZ:00068758</oboInOwl:id>
        <rdfs:label>Lacustrino Pejeperrito Wetlands</rdfs:label>
    </owl:NamedIndividual>
    


    <!-- http://purl.obolibrary.org/obo/GAZ_00068759 -->

    <owl:NamedIndividual rdf:about="http://purl.obolibrary.org/obo/GAZ_00068759">
        <obo:RO_0001025 rdf:resource="http://purl.obolibrary.org/obo/GAZ_00068738"/>
        <obo:IAO_0000115>An area that otects the mouth of the Rio Piro and beach areas on the southern Osa Peninsula, Pacific Coast of Costa Rica.</obo:IAO_0000115>
        <oboInOwl:hasOBONamespace>GAZ</oboInOwl:hasOBONamespace>
        <oboInOwl:id>GAZ:00068759</oboInOwl:id>
        <rdfs:label>Rio Piro Wildlife Refuge</rdfs:label>
    </owl:NamedIndividual>
    


    <!-- http://purl.obolibrary.org/obo/GAZ_00068760 -->

    <owl:NamedIndividual rdf:about="http://purl.obolibrary.org/obo/GAZ_00068760">
        <obo:RO_0001025 rdf:resource="http://purl.obolibrary.org/obo/GAZ_00068738"/>
        <obo:IAO_0000115>An area that protects forested and beach areas on the Golfo Dulce, Pacific Coast of Costa Rica.</obo:IAO_0000115>
        <oboInOwl:hasOBONamespace>GAZ</oboInOwl:hasOBONamespace>
        <oboInOwl:id>GAZ:00068760</oboInOwl:id>
        <rdfs:label>RHR Blancas Wildlife Refuge</rdfs:label>
    </owl:NamedIndividual>
    


    <!-- http://purl.obolibrary.org/obo/GAZ_00068761 -->

    <owl:NamedIndividual rdf:about="http://purl.obolibrary.org/obo/GAZ_00068761">
        <rdf:type rdf:resource="http://purl.obolibrary.org/obo/ENVO_00000004"/>
        <obo:RO_0001025 rdf:resource="http://purl.obolibrary.org/obo/GAZ_00009456"/>
        <obo:IAO_0000115>A district of Golfito Canton.</obo:IAO_0000115>
        <oboInOwl:hasOBONamespace>GAZ</oboInOwl:hasOBONamespace>
        <oboInOwl:id>GAZ:00068761</oboInOwl:id>
        <rdfs:label>Guaycara District</rdfs:label>
    </owl:NamedIndividual>
    


    <!-- http://purl.obolibrary.org/obo/GAZ_00068762 -->

    <owl:NamedIndividual rdf:about="http://purl.obolibrary.org/obo/GAZ_00068762">
        <rdf:type rdf:resource="http://purl.obolibrary.org/obo/ENVO_00000004"/>
        <obo:RO_0001025 rdf:resource="http://purl.obolibrary.org/obo/GAZ_00009456"/>
        <obo:IAO_0000115>A district of Golfito Canton.</obo:IAO_0000115>
        <oboInOwl:hasOBONamespace>GAZ</oboInOwl:hasOBONamespace>
        <oboInOwl:id>GAZ:00068762</oboInOwl:id>
        <rdfs:label>Pavon District</rdfs:label>
    </owl:NamedIndividual>
    


    <!-- http://purl.obolibrary.org/obo/GAZ_00068763 -->

    <owl:NamedIndividual rdf:about="http://purl.obolibrary.org/obo/GAZ_00068763">
        <rdf:type rdf:resource="http://purl.obolibrary.org/obo/ENVO_00000004"/>
        <obo:RO_0001025 rdf:resource="http://purl.obolibrary.org/obo/GAZ_00009456"/>
        <obo:IAO_0000115>A district of Golfito Canton.</obo:IAO_0000115>
        <oboInOwl:hasOBONamespace>GAZ</oboInOwl:hasOBONamespace>
        <oboInOwl:id>GAZ:00068763</oboInOwl:id>
        <rdfs:label>Golfito District</rdfs:label>
    </owl:NamedIndividual>
    


    <!-- http://purl.obolibrary.org/obo/GAZ_00068764 -->

    <owl:NamedIndividual rdf:about="http://purl.obolibrary.org/obo/GAZ_00068764">
        <rdf:type rdf:resource="http://purl.obolibrary.org/obo/ENVO_00000004"/>
        <obo:RO_0001025 rdf:resource="http://purl.obolibrary.org/obo/GAZ_00009456"/>
        <obo:IAO_0000115>A district of Golfito Canton.</obo:IAO_0000115>
        <oboInOwl:hasOBONamespace>GAZ</oboInOwl:hasOBONamespace>
        <oboInOwl:id>GAZ:00068764</oboInOwl:id>
        <rdfs:label>Puerto Jimenez District</rdfs:label>
    </owl:NamedIndividual>
    


    <!-- http://purl.obolibrary.org/obo/GAZ_00068765 -->

    <owl:NamedIndividual rdf:about="http://purl.obolibrary.org/obo/GAZ_00068765">
        <obo:RO_0001025 rdf:resource="http://purl.obolibrary.org/obo/GAZ_00003207"/>
        <obo:IAO_0000115>The 20th canton in the province of San Jose in Costa Rica. The canton covers an area of 120.8 km2. The capital city of the canton is San Pablo. The Quebrada Delicias and the Rio Pirris form major portions of the western and southern boundary, and the Rio Tarrazu establishes the northern and eastern limits of the canton.</obo:IAO_0000115>
        <oboInOwl:hasOBONamespace>GAZ</oboInOwl:hasOBONamespace>
        <oboInOwl:id>GAZ:00068765</oboInOwl:id>
        <rdfs:label>Leon Cortes Canton</rdfs:label>
    </owl:NamedIndividual>
    


    <!-- http://purl.obolibrary.org/obo/GAZ_00068766 -->

    <owl:NamedIndividual rdf:about="http://purl.obolibrary.org/obo/GAZ_00068766">
        <obo:RO_0001025 rdf:resource="http://purl.obolibrary.org/obo/GAZ_00003207"/>
        <obo:IAO_0000115>The second canton in the province of San Jose in Costa Rica. The canton covers an area of 34.49 km2, The capital city of the canton is San Miguel de Escazu, although usually it is called simply Escazu. Although the canton was one of the earliest established in the country, as the metropolitan area has expanded Escazu has become a suburban area on the west side of the national capital city of San Josw. It is delineated by the Rio Tiribi on its northern border. The peak of Cerro Cedral in the Cerros de Escazu marks the southern limit of the canton.</obo:IAO_0000115>
        <oboInOwl:hasOBONamespace>GAZ</oboInOwl:hasOBONamespace>
        <oboInOwl:id>GAZ:00068766</oboInOwl:id>
        <rdfs:label>Escazu Canton</rdfs:label>
    </owl:NamedIndividual>
    


    <!-- http://purl.obolibrary.org/obo/GAZ_00068767 -->

    <owl:NamedIndividual rdf:about="http://purl.obolibrary.org/obo/GAZ_00068767">
        <obo:RO_0001025 rdf:resource="http://purl.obolibrary.org/obo/GAZ_00003207"/>
        <obo:IAO_0000115>The 9th canton in the province of San Jose in Costa Rica. The canton covers an area of 61.42 km2. The capital city of the canton is Santa Ana. The triangular-shaped canton is delineated by the Rio Virilla on the north and stretches south as it narrows to include a portion of the Cerros de Escazu.</obo:IAO_0000115>
        <oboInOwl:hasOBONamespace>GAZ</oboInOwl:hasOBONamespace>
        <oboInOwl:id>GAZ:00068767</oboInOwl:id>
        <rdfs:label>Santa Ana Canton</rdfs:label>
    </owl:NamedIndividual>
    


    <!-- http://purl.obolibrary.org/obo/GAZ_00068768 -->

    <owl:NamedIndividual rdf:about="http://purl.obolibrary.org/obo/GAZ_00068768">
        <obo:RO_0001025 rdf:resource="http://purl.obolibrary.org/obo/GAZ_00003207"/>
        <obo:IAO_0000115>The 3rd canton in the province of San Jose in Costa Rica. The canton covers an area of 118.26 km2. The capital city of the canton is also called Desamparados. The canton begins in the southern suburbs of the national capital city of San Jose, with the Rio Tiribi marking its northern boundary. It snakes its way south in the shape of a backward S, finally reaching its southern limit at the Rio Tarrazu.</obo:IAO_0000115>
        <oboInOwl:hasOBONamespace>GAZ</oboInOwl:hasOBONamespace>
        <oboInOwl:id>GAZ:00068768</oboInOwl:id>
        <rdfs:label>Desamparados Canton</rdfs:label>
    </owl:NamedIndividual>
    


    <!-- http://purl.obolibrary.org/obo/GAZ_00068769 -->

    <owl:NamedIndividual rdf:about="http://purl.obolibrary.org/obo/GAZ_00068769">
        <obo:RO_0001025 rdf:resource="http://purl.obolibrary.org/obo/GAZ_00003207"/>
        <obo:IAO_0000115>The 13th canton in the province of San Jose in Costa Rica. The canton covers an area of 8.15 km2. The capital city of the canton is San Juan. The canton forms a northern suburb of the national capital city of San Jose. It is triangular in shape, with the Rio Virilla as its northern boundary. The Quebrada Rivera, a canyon, establishes the southwestern limit of the canton and also a portion of the southeastern boundary.</obo:IAO_0000115>
        <oboInOwl:hasOBONamespace>GAZ</oboInOwl:hasOBONamespace>
        <oboInOwl:id>GAZ:00068769</oboInOwl:id>
        <rdfs:label>Tibas Canton</rdfs:label>
    </owl:NamedIndividual>
    


    <!-- http://purl.obolibrary.org/obo/GAZ_00068770 -->

    <owl:NamedIndividual rdf:about="http://purl.obolibrary.org/obo/GAZ_00068770">
        <obo:RO_0001025 rdf:resource="http://purl.obolibrary.org/obo/GAZ_00003207"/>
        <obo:IAO_0000115>The 18th canton in the province of San Jose in Costa Rica. The canton covers an area of 15.95 km2. The capital city of the canton is also called Curridabat. The canton forms a suburb of the national capital of San Jose, lying on the southeast edge of the city.</obo:IAO_0000115>
        <oboInOwl:hasOBONamespace>GAZ</oboInOwl:hasOBONamespace>
        <oboInOwl:id>GAZ:00068770</oboInOwl:id>
        <rdfs:label>Curridabat Canton</rdfs:label>
    </owl:NamedIndividual>
    


    <!-- http://purl.obolibrary.org/obo/GAZ_00068771 -->

    <owl:NamedIndividual rdf:about="http://purl.obolibrary.org/obo/GAZ_00068771">
        <obo:RO_0001025 rdf:resource="http://purl.obolibrary.org/obo/GAZ_00003207"/>
        <obo:IAO_0000115>The 14th canton in the province of San Jose in Costa Rica. The canton covers an area of 28.62 km2. The capital city of the canton is San Vincente. The elongated canton begins in the northern suburbs of the national capital city of San Jose and continues northeast toward the Cordillera Central. The Rio Virilla and Rio Para Blanco on the north and west and the Quebrada Azul and Rio Macho on the southeast partially delineate the boundaries of the canton.</obo:IAO_0000115>
        <oboInOwl:hasOBONamespace>GAZ</oboInOwl:hasOBONamespace>
        <oboInOwl:id>GAZ:00068771</oboInOwl:id>
        <rdfs:label>Moravia Canton</rdfs:label>
    </owl:NamedIndividual>
    


    <!-- http://purl.obolibrary.org/obo/GAZ_00068772 -->

    <owl:NamedIndividual rdf:about="http://purl.obolibrary.org/obo/GAZ_00068772">
        <obo:RO_0001025 rdf:resource="http://purl.obolibrary.org/obo/GAZ_00003207"/>
        <obo:IAO_0000115>The 8th canton in the province of San Jose in Costa Rica. The canton covers an area of 31.50 km2. The capital city of the canton is Guadalupe The elongated canton snakes its way through the suburban areas just north of San Jose Centro, climbing steadily into the Cordillera Central until it reaches it eastern limit between the Rio Durazno (on its northern boundary) and the Rio Tiribi (on the south).</obo:IAO_0000115>
        <oboInOwl:hasOBONamespace>GAZ</oboInOwl:hasOBONamespace>
        <oboInOwl:id>GAZ:00068772</oboInOwl:id>
        <rdfs:label>Goicoechea Canton</rdfs:label>
    </owl:NamedIndividual>
    


    <!-- http://purl.obolibrary.org/obo/GAZ_00068773 -->

    <owl:NamedIndividual rdf:about="http://purl.obolibrary.org/obo/GAZ_00068773">
        <obo:RO_0001025 rdf:resource="http://purl.obolibrary.org/obo/GAZ_00003207"/>
        <obo:IAO_0000115>The 11th canton in the province of San Jose in Costa Rica. The canton covers an area of 222.20 km2. The capital city of the canton is San Isidro. The canton of the highlands rises out of the suburbs of San Jose to encompass a major portion of the Cordillera Central and Braulio Carrillo National Park. The Rio Sucio forms the western boundary of the canton, while the Rio Macho, Rio Zurqui and Rio Patria establish the canton&apos;s limits to the east. The northern tip of the canton is marked by the confluence of the Sucio and Patria rivers.</obo:IAO_0000115>
        <oboInOwl:hasOBONamespace>GAZ</oboInOwl:hasOBONamespace>
        <oboInOwl:id>GAZ:00068773</oboInOwl:id>
        <rdfs:label>Vasquez de Coronado Canton</rdfs:label>
    </owl:NamedIndividual>
    


    <!-- http://purl.obolibrary.org/obo/GAZ_00068774 -->

    <owl:NamedIndividual rdf:about="http://purl.obolibrary.org/obo/GAZ_00068774">
        <obo:RO_0001025 rdf:resource="http://purl.obolibrary.org/obo/GAZ_00003207"/>
        <obo:IAO_0000115>The 6th canton in the province of San Jose in Costa Rica. The canton covers an area of 167.10 km2. The capital city of the canton is also called Aserri. The mountainous canton is delineated on the north by the Rio Poas. It encompasses a narrow strip of land that traverses the Coastal Mountain Range before reaching the lowlands of Puntarenas Province, bordering the canton of Parrita.</obo:IAO_0000115>
        <oboInOwl:hasOBONamespace>GAZ</oboInOwl:hasOBONamespace>
        <oboInOwl:id>GAZ:00068774</oboInOwl:id>
        <rdfs:label>Aserri Canton</rdfs:label>
    </owl:NamedIndividual>
    


    <!-- http://purl.obolibrary.org/obo/GAZ_00068775 -->

    <owl:NamedIndividual rdf:about="http://purl.obolibrary.org/obo/GAZ_00068775">
        <obo:RO_0001025 rdf:resource="http://purl.obolibrary.org/obo/GAZ_00003207"/>
        <obo:IAO_0000115>The 16th canton in the province of San Jose in Costa Rica. The canton covers an area of 415.29 km2. The capital city of the canton is San Pablo. The Rio Grande de Tarcoles delineates the north and northwest boundaries of the canton. The Rio Carara, Rio Camaronal and the Fila Negra establish the boundary on the west. The south and southwest is marked by the Rio Tulin, and the Rio Galan and Quebrada Azul delineate portions of the canton&apos;s border on the east.</obo:IAO_0000115>
        <oboInOwl:hasOBONamespace>GAZ</oboInOwl:hasOBONamespace>
        <oboInOwl:id>GAZ:00068775</oboInOwl:id>
        <rdfs:label>Turrubares Canton</rdfs:label>
    </owl:NamedIndividual>
    


    <!-- http://purl.obolibrary.org/obo/GAZ_00068776 -->

    <owl:NamedIndividual rdf:about="http://purl.obolibrary.org/obo/GAZ_00068776">
        <obo:RO_0001025 rdf:resource="http://purl.obolibrary.org/obo/GAZ_00003207"/>
        <obo:IAO_0000115>Thhe 19th canton in the province of San Jose in Costa Rica. The canton covers an area of 1,905.51 km2. The capital city of the canton is San Isidro de El General. The canton&apos;s boundaries are established by the Rio Savegre on the northwest, the Rio Guabo and a series of coastal mountain ranges on the southwest and south, and the peaks of the highest mountains of the Cordillera de Talamanca on the east.</obo:IAO_0000115>
        <oboInOwl:hasOBONamespace>GAZ</oboInOwl:hasOBONamespace>
        <oboInOwl:id>GAZ:00068776</oboInOwl:id>
        <rdfs:label>Perez Zeledon Canton</rdfs:label>
    </owl:NamedIndividual>
    


    <!-- http://purl.obolibrary.org/obo/GAZ_00068777 -->

    <owl:NamedIndividual rdf:about="http://purl.obolibrary.org/obo/GAZ_00068777">
        <obo:RO_0001025 rdf:resource="http://purl.obolibrary.org/obo/GAZ_00003207"/>
        <obo:IAO_0000115>The 5th canton in the province of San Jose in Costa Rica. The canton covers an area of 297.50 km2. The capital city of the canton is San Marcos. The Rio Pirris (also known as Rio Parrita) establishes much of the northern boundary of the three-pronged canton, which reaches south across the Coastal Mountain Range to its border with the canton of Aguirre in Puntarenas Province.</obo:IAO_0000115>
        <oboInOwl:hasOBONamespace>GAZ</oboInOwl:hasOBONamespace>
        <oboInOwl:id>GAZ:00068777</oboInOwl:id>
        <rdfs:label>Tarrazu Canton</rdfs:label>
    </owl:NamedIndividual>
    


    <!-- http://purl.obolibrary.org/obo/GAZ_00068778 -->

    <owl:NamedIndividual rdf:about="http://purl.obolibrary.org/obo/GAZ_00068778">
        <obo:RO_0001025 rdf:resource="http://purl.obolibrary.org/obo/GAZ_00003207"/>
        <obo:IAO_0000115>The 17th canton in the province of San Jose in Costa Rica. The canton covers an area of 400.22 km2. The capital city of the canton is Santa Maria. The canton is delineated by the Rio Savegre on the south and southeast, the Rio Naranjo on the west and the Cordillera de Talamanca on the north and northeast.</obo:IAO_0000115>
        <oboInOwl:hasOBONamespace>GAZ</oboInOwl:hasOBONamespace>
        <oboInOwl:id>GAZ:00068778</oboInOwl:id>
        <rdfs:label>Dota Canton</rdfs:label>
    </owl:NamedIndividual>
    


    <!-- http://purl.obolibrary.org/obo/GAZ_00068779 -->

    <owl:NamedIndividual rdf:about="http://purl.obolibrary.org/obo/GAZ_00068779">
        <obo:RO_0001025 rdf:resource="http://purl.obolibrary.org/obo/GAZ_00003207"/>
        <obo:IAO_0000115>The 7th canton in the province of San Jose in Costa Rica. The canton covers an area of 162.04 km2. The capital city of the canton is Ciudad Colon. The Rio Virilla establishes the northern boundary of the canton, with the Rio Grande de Tarcoles delineating its far western limit. The Rio Chucas, Quebrada Grande, Rio Viejo and Rio Tabarcia mark the canton&apos;s western boundary; the Rio Jorco, Rio Tabarcia and Rio Negro, the southern limit; and a series of foothills rising into the Cerros de Escazu delineate the canton&apos;s eastern border.</obo:IAO_0000115>
        <oboInOwl:hasOBONamespace>GAZ</oboInOwl:hasOBONamespace>
        <oboInOwl:id>GAZ:00068779</oboInOwl:id>
        <rdfs:label>Mora Canton</rdfs:label>
    </owl:NamedIndividual>
    


    <!-- http://purl.obolibrary.org/obo/GAZ_00068780 -->

    <owl:NamedIndividual rdf:about="http://purl.obolibrary.org/obo/GAZ_00068780">
        <obo:RO_0001025 rdf:resource="http://purl.obolibrary.org/obo/GAZ_00003207"/>
        <obo:IAO_0000115>The 15th canton in the province of San Jose in Costa Rica. The canton covers an area of 15.16 km2. The capital city of the canton is San Pedro. The elongated canton reaches from the suburbs of the national capital of San Jose eastward to the province of Cartago, and neighbors the cantons of Curridabat, San Jose, Cartago, and Goicoechea. The Rio Torres delineate a portion of the northern boundary, while the Rio Ocloro and Quebrada Poro mark the southern boundary.</obo:IAO_0000115>
        <oboInOwl:hasOBONamespace>GAZ</oboInOwl:hasOBONamespace>
        <oboInOwl:id>GAZ:00068780</oboInOwl:id>
        <rdfs:label>Montes de Oca Canton</rdfs:label>
    </owl:NamedIndividual>
    


    <!-- http://purl.obolibrary.org/obo/GAZ_00068781 -->

    <owl:NamedIndividual rdf:about="http://purl.obolibrary.org/obo/GAZ_00068781">
        <obo:RO_0001025 rdf:resource="http://purl.obolibrary.org/obo/GAZ_00003207"/>
        <obo:IAO_0000115>The 4th canton in the province of San Jose in Costa Rica. The canton covers an area of 553.66 km2. The capital city of the canton is Santiago. The Rio Chucas delineates the canton&apos;s northernmost boundary, while the Rio Chires marks its far southern border with the Puntarenas canton of Parrita. The canton includes a major portion of the Coastal Mountain Range.</obo:IAO_0000115>
        <oboInOwl:hasOBONamespace>GAZ</oboInOwl:hasOBONamespace>
        <oboInOwl:id>GAZ:00068781</oboInOwl:id>
        <rdfs:label>Puriscal Canton</rdfs:label>
    </owl:NamedIndividual>
    


    <!-- http://purl.obolibrary.org/obo/GAZ_00068782 -->

    <owl:NamedIndividual rdf:about="http://purl.obolibrary.org/obo/GAZ_00068782">
        <obo:RO_0001025 rdf:resource="http://purl.obolibrary.org/obo/GAZ_00003207"/>
        <obo:IAO_0000115>The 12th canton in the province of San Jose in Costa Rica. The canton covers an area of 242.24 km2. The capital city of the canton is San Ignacio. The mountainous canton begins in the Cerros de Escazu on the far western edge of the San Jose Metropolitan Area. It continues west and south between the Rio Negro on the north and the Rio Jorco on the east to encompass a large portion of the Coastal Mountain Range, finally ending at the border of Puntarenas Province near the Pacific coast in Parrita Canton.</obo:IAO_0000115>
        <oboInOwl:hasOBONamespace>GAZ</oboInOwl:hasOBONamespace>
        <oboInOwl:id>GAZ:00068782</oboInOwl:id>
        <rdfs:label>Acosta Canton</rdfs:label>
    </owl:NamedIndividual>
    


    <!-- http://purl.obolibrary.org/obo/GAZ_00068783 -->

    <owl:NamedIndividual rdf:about="http://purl.obolibrary.org/obo/GAZ_00068783">
        <obo:RO_0001025 rdf:resource="http://purl.obolibrary.org/obo/GAZ_00003207"/>
        <obo:IAO_0000115>The 10th canton in the province of San Jose in Costa Rica. The canton covers an area of 21.17 km2. The capital city of the canton is Alajuelita. The odd-shaped canton reaches southwest from the suburbs of the national capital city of San Jose. It is delineated by the Rio Tiribi on the northeast, Rio Canas on the east, Rio Poas on the southeast, and the Cerros de Escazu at it far southwestern end.</obo:IAO_0000115>
        <oboInOwl:hasOBONamespace>GAZ</oboInOwl:hasOBONamespace>
        <oboInOwl:id>GAZ:00068783</oboInOwl:id>
        <rdfs:label>Alajuelita Canton</rdfs:label>
    </owl:NamedIndividual>
    


    <!-- http://purl.obolibrary.org/obo/GAZ_00068784 -->

    <owl:NamedIndividual rdf:about="http://purl.obolibrary.org/obo/GAZ_00068784">
        <rdf:type rdf:resource="http://purl.obolibrary.org/obo/ENVO_00000004"/>
        <obo:RO_0001025 rdf:resource="http://purl.obolibrary.org/obo/GAZ_00007745"/>
        <obo:IAO_0000115>A district of San Jose Canton.</obo:IAO_0000115>
        <oboInOwl:hasOBONamespace>GAZ</oboInOwl:hasOBONamespace>
        <oboInOwl:id>GAZ:00068784</oboInOwl:id>
        <rdfs:label>Mata Redonda District</rdfs:label>
    </owl:NamedIndividual>
    


    <!-- http://purl.obolibrary.org/obo/GAZ_00068785 -->

    <owl:NamedIndividual rdf:about="http://purl.obolibrary.org/obo/GAZ_00068785">
        <rdf:type rdf:resource="http://purl.obolibrary.org/obo/ENVO_00000004"/>
        <obo:RO_0001025 rdf:resource="http://purl.obolibrary.org/obo/GAZ_00007745"/>
        <obo:IAO_0000115>A district of San Jose Canton.</obo:IAO_0000115>
        <oboInOwl:hasOBONamespace>GAZ</oboInOwl:hasOBONamespace>
        <oboInOwl:id>GAZ:00068785</oboInOwl:id>
        <rdfs:label>San Sebastian District</rdfs:label>
    </owl:NamedIndividual>
    


    <!-- http://purl.obolibrary.org/obo/GAZ_00068786 -->

    <owl:NamedIndividual rdf:about="http://purl.obolibrary.org/obo/GAZ_00068786">
        <rdf:type rdf:resource="http://purl.obolibrary.org/obo/ENVO_00000004"/>
        <obo:RO_0001025 rdf:resource="http://purl.obolibrary.org/obo/GAZ_00007745"/>
        <obo:IAO_0000115>A district of San Jose Canton.</obo:IAO_0000115>
        <oboInOwl:hasOBONamespace>GAZ</oboInOwl:hasOBONamespace>
        <oboInOwl:id>GAZ:00068786</oboInOwl:id>
        <rdfs:label>Hatillo District</rdfs:label>
    </owl:NamedIndividual>
    


    <!-- http://purl.obolibrary.org/obo/GAZ_00068787 -->

    <owl:NamedIndividual rdf:about="http://purl.obolibrary.org/obo/GAZ_00068787">
        <obo:RO_0001025 rdf:resource="http://purl.obolibrary.org/obo/GAZ_00007745"/>
        <obo:IAO_0000115>The sixth &quot;distrito&quot; of San Jose Canton, Costa Rica, is one of the administrative units surrounding San Jose downtown. San Francisco de Dos Rios lies on the south-east of the canton, between Curridabat and Desamparados cantons (bordering them to the east and to the south respectively) and between the josefino districts of San Sebastian and Catedral (bordering them also to the west and to the north respectively).</obo:IAO_0000115>
        <oboInOwl:hasOBONamespace>GAZ</oboInOwl:hasOBONamespace>
        <oboInOwl:id>GAZ:00068787</oboInOwl:id>
        <rdfs:label>San Francisco de Dos Rios District</rdfs:label>
    </owl:NamedIndividual>
    


    <!-- http://purl.obolibrary.org/obo/GAZ_00068788 -->

    <owl:NamedIndividual rdf:about="http://purl.obolibrary.org/obo/GAZ_00068788">
        <obo:RO_0001025 rdf:resource="http://purl.obolibrary.org/obo/GAZ_00007745"/>
        <obo:IAO_0000115>The second &quot;distrito&quot; of San Jose Canton, in Costa Rica, is one of the four administrative units that form San Jose downtown properly. Merced District lies in the north of the canton, limiting only with Tibas Canton from San Jose Province to the north, and with the districts of Uruca to the north, Mata Redonda to the west, Hospital to the south, and Uruca and El Carmen &quot;distritos&quot; to the east, all of them from the same canton of San Jose.</obo:IAO_0000115>
        <oboInOwl:hasOBONamespace>GAZ</oboInOwl:hasOBONamespace>
        <oboInOwl:id>GAZ:00068788</oboInOwl:id>
        <rdfs:label>Merced District</rdfs:label>
    </owl:NamedIndividual>
    


    <!-- http://purl.obolibrary.org/obo/GAZ_00068789 -->

    <owl:NamedIndividual rdf:about="http://purl.obolibrary.org/obo/GAZ_00068789">
        <obo:RO_0001025 rdf:resource="http://purl.obolibrary.org/obo/GAZ_00007745"/>
        <obo:IAO_0000115>The first &quot;distrito&quot; of San Jose Canton, in Costa Rica, and one of the four administrative units that form San Jose city properly. El Carmen District lies in the north of the canton, limiting (clockwise) with Goicoechea Canton and Montes de Oca Canton from San Jose Province at the north and east respectively. The District also limits with other districts of San Jose Canton, Catedral district at the south and Merced District at the west.</obo:IAO_0000115>
        <oboInOwl:hasOBONamespace>GAZ</oboInOwl:hasOBONamespace>
        <oboInOwl:id>GAZ:00068789</oboInOwl:id>
        <rdfs:label>El Carmen District</rdfs:label>
    </owl:NamedIndividual>
    


    <!-- http://purl.obolibrary.org/obo/GAZ_00068790 -->

    <owl:NamedIndividual rdf:about="http://purl.obolibrary.org/obo/GAZ_00068790">
        <rdf:type rdf:resource="http://purl.obolibrary.org/obo/ENVO_00000004"/>
        <obo:RO_0001025 rdf:resource="http://purl.obolibrary.org/obo/GAZ_00007745"/>
        <obo:IAO_0000115>A district of San Jose Canton.</obo:IAO_0000115>
        <oboInOwl:hasOBONamespace>GAZ</oboInOwl:hasOBONamespace>
        <oboInOwl:id>GAZ:00068790</oboInOwl:id>
        <rdfs:label>Pavas District</rdfs:label>
    </owl:NamedIndividual>
    


    <!-- http://purl.obolibrary.org/obo/GAZ_00068791 -->

    <owl:NamedIndividual rdf:about="http://purl.obolibrary.org/obo/GAZ_00068791">
        <obo:RO_0001025 rdf:resource="http://purl.obolibrary.org/obo/GAZ_00007745"/>
        <obo:IAO_0000115>The fourth &quot;distrito&quot; of San Jose Canton, Costa Rica, is one of the four administrative units that form San Jose downtown properly. Catedral District is on the center-east of the canton, and has a small portion of boundary with Montes de Oca Canton at its eastern part. The division also borders (clockwards) Zapote district to the east, San Sebastian district to the south, Hospital and Merced districts to the west, and El Carmen district to the north.</obo:IAO_0000115>
        <oboInOwl:hasOBONamespace>GAZ</oboInOwl:hasOBONamespace>
        <oboInOwl:id>GAZ:00068791</oboInOwl:id>
        <rdfs:label>Catedral District</rdfs:label>
    </owl:NamedIndividual>
    


    <!-- http://purl.obolibrary.org/obo/GAZ_00068792 -->

    <owl:NamedIndividual rdf:about="http://purl.obolibrary.org/obo/GAZ_00068792">
        <obo:RO_0001025 rdf:resource="http://purl.obolibrary.org/obo/GAZ_00007745"/>
        <obo:IAO_0000115>The third &quot;distrito&quot; of San Jose Canton, Costa Rica, and is one of the four administrative units that form San Jose downtown properly. Hospital District lies in the center of the canton, the only one which limits with districts of San Jose and not with other cantons. The district borders (clockwards) with Merced district to the north, El Carmen and Catedral districts to the east, San Sebastian and Hatillo districts to the south, and Mata Redonda district to the west.</obo:IAO_0000115>
        <oboInOwl:hasOBONamespace>GAZ</oboInOwl:hasOBONamespace>
        <oboInOwl:id>GAZ:00068792</oboInOwl:id>
        <rdfs:label>Hospital District</rdfs:label>
    </owl:NamedIndividual>
    


    <!-- http://purl.obolibrary.org/obo/GAZ_00068793 -->

    <owl:NamedIndividual rdf:about="http://purl.obolibrary.org/obo/GAZ_00068793">
        <obo:RO_0001025 rdf:resource="http://purl.obolibrary.org/obo/GAZ_00007745"/>
        <obo:IAO_0000115>The fifth &quot;distrito&quot; of San Jose Canton, Costa Rica, is one of the administrative units surrounding San Jose downtown. Zapote is on the east of the canton, lying between Montes de Oca Canton and Curridabat Canton (bordering them to the north and to the east respectively). The district also borders San Francisco district to the south, and Catedral district to the west.</obo:IAO_0000115>
        <oboInOwl:hasOBONamespace>GAZ</oboInOwl:hasOBONamespace>
        <oboInOwl:id>GAZ:00068793</oboInOwl:id>
        <rdfs:label>Zapote District</rdfs:label>
    </owl:NamedIndividual>
    


    <!-- http://purl.obolibrary.org/obo/GAZ_00068794 -->

    <owl:NamedIndividual rdf:about="http://purl.obolibrary.org/obo/GAZ_00068794">
        <rdf:type rdf:resource="http://purl.obolibrary.org/obo/ENVO_00000004"/>
        <obo:RO_0001025 rdf:resource="http://purl.obolibrary.org/obo/GAZ_00007745"/>
        <obo:IAO_0000115>A district of San Jose Canton.</obo:IAO_0000115>
        <oboInOwl:hasOBONamespace>GAZ</oboInOwl:hasOBONamespace>
        <oboInOwl:id>GAZ:00068794</oboInOwl:id>
        <rdfs:label>Uruca District</rdfs:label>
    </owl:NamedIndividual>
    


    <!-- http://purl.obolibrary.org/obo/GAZ_00068795 -->

    <owl:NamedIndividual rdf:about="http://purl.obolibrary.org/obo/GAZ_00068795">
        <obo:RO_0001025 rdf:resource="http://purl.obolibrary.org/obo/GAZ_00003207"/>
        <obo:IAO_0000115>A mountain range in central Costa Rica. It borders the Central Valley to the south and is considered the northernmost portion of the Cordillera de Talamanca.</obo:IAO_0000115>
        <oboInOwl:hasOBONamespace>GAZ</oboInOwl:hasOBONamespace>
        <oboInOwl:id>GAZ:00068795</oboInOwl:id>
        <rdfs:label>Cerros de Escazu</rdfs:label>
    </owl:NamedIndividual>
    


    <!-- http://purl.obolibrary.org/obo/GAZ_00068796 -->

    <owl:NamedIndividual rdf:about="http://purl.obolibrary.org/obo/GAZ_00068796">
        <obo:RO_0001025 rdf:resource="http://purl.obolibrary.org/obo/GAZ_00003210"/>
        <obo:RO_0001025 rdf:resource="http://purl.obolibrary.org/obo/GAZ_00068682"/>
        <obo:IAO_0000115>A protected area with the Tempisque Conservation Area.</obo:IAO_0000115>
        <oboInOwl:hasOBONamespace>GAZ</oboInOwl:hasOBONamespace>
        <oboInOwl:id>GAZ:00068796</oboInOwl:id>
        <rdfs:label>Laguna Madrigal Wetlands</rdfs:label>
    </owl:NamedIndividual>
    


    <!-- http://purl.obolibrary.org/obo/GAZ_00068797 -->

    <owl:NamedIndividual rdf:about="http://purl.obolibrary.org/obo/GAZ_00068797">
        <obo:RO_0001025 rdf:resource="http://purl.obolibrary.org/obo/GAZ_00003210"/>
        <obo:RO_0001025 rdf:resource="http://purl.obolibrary.org/obo/GAZ_00068682"/>
        <obo:IAO_0000115>A protected area with the Tempisque Conservation Area.</obo:IAO_0000115>
        <oboInOwl:hasOBONamespace>GAZ</oboInOwl:hasOBONamespace>
        <oboInOwl:id>GAZ:00068797</oboInOwl:id>
        <rdfs:label>Finca La Virgen</rdfs:label>
    </owl:NamedIndividual>
    


    <!-- http://purl.obolibrary.org/obo/GAZ_00068798 -->

    <owl:NamedIndividual rdf:about="http://purl.obolibrary.org/obo/GAZ_00068798">
        <obo:RO_0001025 rdf:resource="http://purl.obolibrary.org/obo/GAZ_00003210"/>
        <obo:RO_0001025 rdf:resource="http://purl.obolibrary.org/obo/GAZ_00068682"/>
        <obo:IAO_0000115>A protected area with the Tempisque Conservation Area.</obo:IAO_0000115>
        <oboInOwl:hasOBONamespace>GAZ</oboInOwl:hasOBONamespace>
        <oboInOwl:id>GAZ:00068798</oboInOwl:id>
        <rdfs:label>Cerro La Cruz Protected Zone</rdfs:label>
    </owl:NamedIndividual>
    


    <!-- http://purl.obolibrary.org/obo/GAZ_00068799 -->

    <owl:NamedIndividual rdf:about="http://purl.obolibrary.org/obo/GAZ_00068799">
        <obo:RO_0001025 rdf:resource="http://purl.obolibrary.org/obo/GAZ_00003210"/>
        <obo:RO_0001025 rdf:resource="http://purl.obolibrary.org/obo/GAZ_00068682"/>
        <obo:IAO_0000115>A wildlife refuge of Costa Rica, part of the Tempisque Conservation Area, protects the estuary and river mouth of the Matapalo River near the Las Baulas National Marine Park.</obo:IAO_0000115>
        <oboInOwl:hasOBONamespace>GAZ</oboInOwl:hasOBONamespace>
        <oboInOwl:id>GAZ:00068799</oboInOwl:id>
        <rdfs:label>Tamarindo Wildlife Refuge</rdfs:label>
    </owl:NamedIndividual>
    


    <!-- http://purl.obolibrary.org/obo/GAZ_00068800 -->

    <owl:NamedIndividual rdf:about="http://purl.obolibrary.org/obo/GAZ_00068800">
        <obo:RO_0001025 rdf:resource="http://purl.obolibrary.org/obo/GAZ_00003210"/>
        <obo:RO_0001025 rdf:resource="http://purl.obolibrary.org/obo/GAZ_00068682"/>
        <obo:IAO_0000115>A protected area with the Tempisque Conservation Area.</obo:IAO_0000115>
        <oboInOwl:hasOBONamespace>GAZ</oboInOwl:hasOBONamespace>
        <oboInOwl:id>GAZ:00068800</oboInOwl:id>
        <rdfs:label>Nosara Protected Zone</rdfs:label>
    </owl:NamedIndividual>
    


    <!-- http://purl.obolibrary.org/obo/GAZ_00068801 -->

    <owl:NamedIndividual rdf:about="http://purl.obolibrary.org/obo/GAZ_00068801">
        <obo:RO_0001025 rdf:resource="http://purl.obolibrary.org/obo/GAZ_00068682"/>
        <obo:RO_0001025 rdf:resource="http://purl.obolibrary.org/obo/GAZ_00068699"/>
        <obo:IAO_0000115>A nature reserve, part of the Guanacaste Conservation Area and Tempisque Conservation Area in northwestern Costa Rica, which protects low wetlands around the Quebrada Grande and the Ahogados River in the Tempisque River watershed.</obo:IAO_0000115>
        <oboInOwl:hasOBONamespace>GAZ</oboInOwl:hasOBONamespace>
        <oboInOwl:id>GAZ:00068801</oboInOwl:id>
        <rdfs:label>Riberino Zapandi Wetlands</rdfs:label>
    </owl:NamedIndividual>
    


    <!-- http://purl.obolibrary.org/obo/GAZ_00068802 -->

    <owl:NamedIndividual rdf:about="http://purl.obolibrary.org/obo/GAZ_00068802">
        <obo:RO_0001025 rdf:resource="http://purl.obolibrary.org/obo/GAZ_00003210"/>
        <obo:RO_0001025 rdf:resource="http://purl.obolibrary.org/obo/GAZ_00068682"/>
        <obo:IAO_0000115>A protected area with the Tempisque Conservation Area.</obo:IAO_0000115>
        <oboInOwl:hasOBONamespace>GAZ</oboInOwl:hasOBONamespace>
        <oboInOwl:id>GAZ:00068802</oboInOwl:id>
        <rdfs:label>Palustrino Corral de Piedra Wetlands</rdfs:label>
    </owl:NamedIndividual>
    


    <!-- http://purl.obolibrary.org/obo/GAZ_00068803 -->

    <owl:NamedIndividual rdf:about="http://purl.obolibrary.org/obo/GAZ_00068803">
        <obo:RO_0001025 rdf:resource="http://purl.obolibrary.org/obo/GAZ_00068682"/>
        <obo:RO_0001025 rdf:resource="http://purl.obolibrary.org/obo/GAZ_00068690"/>
        <obo:IAO_0000115>A nature reserve of Costa Rica, part of the Tempisque Conservation Area, comprising of two islands separated by a small channel in the Gulf of Nicoya which protects migratory bird species which use the island seasonally.</obo:IAO_0000115>
        <oboInOwl:hasOBONamespace>GAZ</oboInOwl:hasOBONamespace>
        <oboInOwl:id>GAZ:00068803</oboInOwl:id>
        <rdfs:label>Negritos Islands Biological Reserve</rdfs:label>
    </owl:NamedIndividual>
    


    <!-- http://purl.obolibrary.org/obo/GAZ_00068804 -->

    <owl:NamedIndividual rdf:about="http://purl.obolibrary.org/obo/GAZ_00068804">
        <obo:RO_0001025 rdf:resource="http://purl.obolibrary.org/obo/GAZ_00003210"/>
        <obo:RO_0001025 rdf:resource="http://purl.obolibrary.org/obo/GAZ_00068682"/>
        <obo:IAO_0000115>A protected area with the Tempisque Conservation Area.</obo:IAO_0000115>
        <oboInOwl:hasOBONamespace>GAZ</oboInOwl:hasOBONamespace>
        <oboInOwl:id>GAZ:00068804</oboInOwl:id>
        <rdfs:label>Cuenca Rio Abangares Protected Zone</rdfs:label>
    </owl:NamedIndividual>
    


    <!-- http://purl.obolibrary.org/obo/GAZ_00068805 -->

    <owl:NamedIndividual rdf:about="http://purl.obolibrary.org/obo/GAZ_00068805">
        <obo:RO_0001025 rdf:resource="http://purl.obolibrary.org/obo/GAZ_00003210"/>
        <obo:RO_0001025 rdf:resource="http://purl.obolibrary.org/obo/GAZ_00068682"/>
        <obo:IAO_0000115>A protected area with the Tempisque Conservation Area.</obo:IAO_0000115>
        <oboInOwl:hasOBONamespace>GAZ</oboInOwl:hasOBONamespace>
        <oboInOwl:id>GAZ:00068805</oboInOwl:id>
        <rdfs:label>Rio Canas Wetlands</rdfs:label>
    </owl:NamedIndividual>
    


    <!-- http://purl.obolibrary.org/obo/GAZ_00068806 -->

    <owl:NamedIndividual rdf:about="http://purl.obolibrary.org/obo/GAZ_00068806">
        <obo:RO_0001025 rdf:resource="http://purl.obolibrary.org/obo/GAZ_00068681"/>
        <obo:RO_0001025 rdf:resource="http://purl.obolibrary.org/obo/GAZ_00068682"/>
        <obo:IAO_0000115>A protected area with the Tempisque Conservation Area.</obo:IAO_0000115>
        <oboInOwl:hasOBONamespace>GAZ</oboInOwl:hasOBONamespace>
        <oboInOwl:id>GAZ:00068806</oboInOwl:id>
        <rdfs:label>Nicoya Peninsula Protected Zone</rdfs:label>
    </owl:NamedIndividual>
    


    <!-- http://purl.obolibrary.org/obo/GAZ_00068807 -->

    <owl:NamedIndividual rdf:about="http://purl.obolibrary.org/obo/GAZ_00068807">
        <obo:RO_0001025 rdf:resource="http://purl.obolibrary.org/obo/GAZ_00003210"/>
        <obo:RO_0001025 rdf:resource="http://purl.obolibrary.org/obo/GAZ_00068682"/>
        <obo:IAO_0000115>A protected area with the Tempisque Conservation Area.</obo:IAO_0000115>
        <oboInOwl:hasOBONamespace>GAZ</oboInOwl:hasOBONamespace>
        <oboInOwl:id>GAZ:00068807</oboInOwl:id>
        <rdfs:label>Werner Sauter Wildlife Refuge</rdfs:label>
    </owl:NamedIndividual>
    


    <!-- http://purl.obolibrary.org/obo/GAZ_00068808 -->

    <owl:NamedIndividual rdf:about="http://purl.obolibrary.org/obo/GAZ_00068808">
        <obo:RO_0001025 rdf:resource="http://purl.obolibrary.org/obo/GAZ_00003210"/>
        <obo:RO_0001025 rdf:resource="http://purl.obolibrary.org/obo/GAZ_00068682"/>
        <obo:IAO_0000115>A protected area with the Tempisque Conservation Area.</obo:IAO_0000115>
        <oboInOwl:hasOBONamespace>GAZ</oboInOwl:hasOBONamespace>
        <oboInOwl:id>GAZ:00068808</oboInOwl:id>
        <rdfs:label>Costa Esmeralda Wildlife Refuge</rdfs:label>
    </owl:NamedIndividual>
    


    <!-- http://purl.obolibrary.org/obo/GAZ_00068809 -->

    <owl:NamedIndividual rdf:about="http://purl.obolibrary.org/obo/GAZ_00068809">
        <obo:RO_0001025 rdf:resource="http://purl.obolibrary.org/obo/GAZ_00068681"/>
        <obo:RO_0001025 rdf:resource="http://purl.obolibrary.org/obo/GAZ_00068682"/>
        <obo:IAO_0000115>A protected area with the Tempisque Conservation Area.</obo:IAO_0000115>
        <oboInOwl:hasOBONamespace>GAZ</oboInOwl:hasOBONamespace>
        <oboInOwl:id>GAZ:00068809</oboInOwl:id>
        <rdfs:label>Nicolas Wessberg Absolute Natural Reserve</rdfs:label>
    </owl:NamedIndividual>
    


    <!-- http://purl.obolibrary.org/obo/GAZ_00068810 -->

    <owl:NamedIndividual rdf:about="http://purl.obolibrary.org/obo/GAZ_00068810">
        <obo:RO_0001025 rdf:resource="http://purl.obolibrary.org/obo/GAZ_00003210"/>
        <obo:RO_0001025 rdf:resource="http://purl.obolibrary.org/obo/GAZ_00068682"/>
        <obo:IAO_0000115>A protected area with the Tempisque Conservation Area.</obo:IAO_0000115>
        <oboInOwl:hasOBONamespace>GAZ</oboInOwl:hasOBONamespace>
        <oboInOwl:id>GAZ:00068810</oboInOwl:id>
        <rdfs:label>Taboga Forest Reserve</rdfs:label>
    </owl:NamedIndividual>
    


    <!-- http://purl.obolibrary.org/obo/GAZ_00068811 -->

    <owl:NamedIndividual rdf:about="http://purl.obolibrary.org/obo/GAZ_00068811">
        <obo:RO_0001025 rdf:resource="http://purl.obolibrary.org/obo/GAZ_00003210"/>
        <obo:RO_0001025 rdf:resource="http://purl.obolibrary.org/obo/GAZ_00068682"/>
        <obo:IAO_0000115>A wildlife refuge of Costa Rica, part of the Tempisque Conservation Area, was originally declared a protected area in 1982, and its status has been changed several times since then, including covering a larger area both on land and out to sea.</obo:IAO_0000115>
        <oboInOwl:hasOBONamespace>GAZ</oboInOwl:hasOBONamespace>
        <oboInOwl:id>GAZ:00068811</oboInOwl:id>
        <rdfs:label>Ostional Wildlife Refuge</rdfs:label>
    </owl:NamedIndividual>
    


    <!-- http://purl.obolibrary.org/obo/GAZ_00068812 -->

    <owl:NamedIndividual rdf:about="http://purl.obolibrary.org/obo/GAZ_00068812">
        <obo:RO_0001025 rdf:resource="http://purl.obolibrary.org/obo/GAZ_00068682"/>
        <obo:IAO_0000115>A national park of Costa Rica, part of the Tempisque Conservation Area, that contains much of the area of the valley of the Tempisque River and covers an area of 45,492 acres in Guanacaste Province, 30 km west of Canas.</obo:IAO_0000115>
        <oboInOwl:hasOBONamespace>GAZ</oboInOwl:hasOBONamespace>
        <oboInOwl:id>GAZ:00068812</oboInOwl:id>
        <rdfs:label>Parque Nacional Palo Verde</rdfs:label>
    </owl:NamedIndividual>
    


    <!-- http://purl.obolibrary.org/obo/GAZ_00068813 -->

    <owl:NamedIndividual rdf:about="http://purl.obolibrary.org/obo/GAZ_00068813">
        <obo:RO_0001025 rdf:resource="http://purl.obolibrary.org/obo/GAZ_00003210"/>
        <obo:RO_0001025 rdf:resource="http://purl.obolibrary.org/obo/GAZ_00068682"/>
        <obo:IAO_0000115>A nature reserve of Costa Rica, part of the Tempisque Conservation Area, and covers approximately 220 km2 marine near the town of Tamarindo.</obo:IAO_0000115>
        <oboInOwl:hasOBONamespace>GAZ</oboInOwl:hasOBONamespace>
        <oboInOwl:id>GAZ:00068813</oboInOwl:id>
        <rdfs:label>Parque Nacional Marino Las Baulas</rdfs:label>
    </owl:NamedIndividual>
    


    <!-- http://purl.obolibrary.org/obo/GAZ_00068814 -->

    <owl:NamedIndividual rdf:about="http://purl.obolibrary.org/obo/GAZ_00068814">
        <obo:RO_0001025 rdf:resource="http://purl.obolibrary.org/obo/GAZ_00068682"/>
        <obo:RO_0001025 rdf:resource="http://purl.obolibrary.org/obo/GAZ_00068690"/>
        <obo:IAO_0000115>A nature reserve of Costa Rica, part of the Tempisque Conservation Area, which encompasses the four islands including Guayabo and Los Pajaros in the Gulf of Nicoya.</obo:IAO_0000115>
        <oboInOwl:hasOBONamespace>GAZ</oboInOwl:hasOBONamespace>
        <oboInOwl:id>GAZ:00068814</oboInOwl:id>
        <rdfs:label>Guayabo Islands Biological Reserve</rdfs:label>
    </owl:NamedIndividual>
    


    <!-- http://purl.obolibrary.org/obo/GAZ_00068815 -->

    <owl:NamedIndividual rdf:about="http://purl.obolibrary.org/obo/GAZ_00068815">
        <obo:RO_0001025 rdf:resource="http://purl.obolibrary.org/obo/GAZ_00068681"/>
        <obo:RO_0001025 rdf:resource="http://purl.obolibrary.org/obo/GAZ_00068682"/>
        <obo:IAO_0000115>A wildlife refuge of Costa Rica, part of the Tempisque Conservation Area, which protects tropical forest and wetlands near the Tempisque River and the town of Rosario.</obo:IAO_0000115>
        <oboInOwl:hasOBONamespace>GAZ</oboInOwl:hasOBONamespace>
        <oboInOwl:id>GAZ:00068815</oboInOwl:id>
        <rdfs:label>Mata Redonda Wildlife Refuge</rdfs:label>
    </owl:NamedIndividual>
    


    <!-- http://purl.obolibrary.org/obo/GAZ_00068816 -->

    <owl:NamedIndividual rdf:about="http://purl.obolibrary.org/obo/GAZ_00068816">
        <obo:RO_0001025 rdf:resource="http://purl.obolibrary.org/obo/GAZ_00003210"/>
        <obo:RO_0001025 rdf:resource="http://purl.obolibrary.org/obo/GAZ_00068682"/>
        <obo:IAO_0000115>A wildlife refuge of Costa Rica, part of the Tempisque Conservation Area, and protects tropical forest and wetlands on the banks of the Tempisque River near Abangares in the Guanacaste Province.</obo:IAO_0000115>
        <oboInOwl:hasOBONamespace>GAZ</oboInOwl:hasOBONamespace>
        <oboInOwl:id>GAZ:00068816</oboInOwl:id>
        <rdfs:label>Cipanci Wildlife Refuge</rdfs:label>
    </owl:NamedIndividual>
    


    <!-- http://purl.obolibrary.org/obo/GAZ_00068817 -->

    <owl:NamedIndividual rdf:about="http://purl.obolibrary.org/obo/GAZ_00068817">
        <obo:RO_0001025 rdf:resource="http://purl.obolibrary.org/obo/GAZ_00003210"/>
        <obo:RO_0001025 rdf:resource="http://purl.obolibrary.org/obo/GAZ_00068682"/>
        <obo:IAO_0000115>A nature reserve of Costa Rica, part of the Tempisque Conservation Area, that covers an area of 26 km2 in the Guanacaste Province, 15 km southwest of Bagaces. The Barbudal Lomas are ignimbritic plateaux which end in rocky cliffs that rise to 125 m above the Tempisque River.</obo:IAO_0000115>
        <oboInOwl:hasOBONamespace>GAZ</oboInOwl:hasOBONamespace>
        <oboInOwl:id>GAZ:00068817</oboInOwl:id>
        <rdfs:label>Lomas de Barbudal Biological Reserve</rdfs:label>
    </owl:NamedIndividual>
    


    <!-- http://purl.obolibrary.org/obo/GAZ_00068818 -->

    <owl:NamedIndividual rdf:about="http://purl.obolibrary.org/obo/GAZ_00068818">
        <obo:RO_0001025 rdf:resource="http://purl.obolibrary.org/obo/GAZ_00068814"/>
        <obo:IAO_0000115>An island found in the northern end of Gigante Bay, Guayabo Island is a 6.8 ha rocky islet with high cliffs and little vegetation.</obo:IAO_0000115>
        <oboInOwl:hasOBONamespace>GAZ</oboInOwl:hasOBONamespace>
        <oboInOwl:id>GAZ:00068818</oboInOwl:id>
        <rdfs:label>Isla Guayabo</rdfs:label>
    </owl:NamedIndividual>
    


    <!-- http://purl.obolibrary.org/obo/GAZ_00068819 -->

    <owl:NamedIndividual rdf:about="http://purl.obolibrary.org/obo/GAZ_00068819">
        <obo:RO_0001025 rdf:resource="http://purl.obolibrary.org/obo/GAZ_00068850"/>
        <oboInOwl:hasOBONamespace>GAZ</oboInOwl:hasOBONamespace>
        <oboInOwl:id>GAZ:00068819</oboInOwl:id>
        <rdfs:label>Los Pajaros</rdfs:label>
    </owl:NamedIndividual>
    


    <!-- http://purl.obolibrary.org/obo/GAZ_00068820 -->

    <owl:NamedIndividual rdf:about="http://purl.obolibrary.org/obo/GAZ_00068820">
        <obo:RO_0001025 rdf:resource="http://purl.obolibrary.org/obo/GAZ_00068699"/>
        <obo:RO_0001025 rdf:resource="http://purl.obolibrary.org/obo/GAZ_00068826"/>
        <obo:RO_0001025 rdf:resource="http://purl.obolibrary.org/obo/GAZ_00068836"/>
        <obo:RO_0001025 rdf:resource="http://purl.obolibrary.org/obo/GAZ_00068897"/>
        <obo:IAO_0000115>A wildlife refuge, running through Arenal Huetar Norte, Guanacaste, Central Volcanic and Tortuguero Conservation Areas, in the northern part of Costa Rica running as a 2,000 m wide strip of land along the border with Nicaragua. It was created in 1994.</obo:IAO_0000115>
        <oboInOwl:hasOBONamespace>GAZ</oboInOwl:hasOBONamespace>
        <oboInOwl:id>GAZ:00068820</oboInOwl:id>
        <rdfs:label>Corredor Fronterizo Wildlife Refuge</rdfs:label>
    </owl:NamedIndividual>
    


    <!-- http://purl.obolibrary.org/obo/GAZ_00068821 -->

    <owl:NamedIndividual rdf:about="http://purl.obolibrary.org/obo/GAZ_00068821">
        <obo:RO_0001025 rdf:resource="http://purl.obolibrary.org/obo/GAZ_00003210"/>
        <obo:RO_0001025 rdf:resource="http://purl.obolibrary.org/obo/GAZ_00068699"/>
        <obo:IAO_0000115>A wildlife refuge, part of the Guanacaste Conservation Area, in northwestern Costa Rica. It protects coastal mangroves and areas around the Quebrada Grande.</obo:IAO_0000115>
        <oboInOwl:hasOBONamespace>GAZ</oboInOwl:hasOBONamespace>
        <oboInOwl:id>GAZ:00068821</oboInOwl:id>
        <rdfs:label>Iguanita Wildlife Refuge</rdfs:label>
    </owl:NamedIndividual>
    


    <!-- http://purl.obolibrary.org/obo/GAZ_00068822 -->

    <owl:NamedIndividual rdf:about="http://purl.obolibrary.org/obo/GAZ_00068822">
        <obo:RO_0001025 rdf:resource="http://purl.obolibrary.org/obo/GAZ_00003210"/>
        <obo:RO_0001025 rdf:resource="http://purl.obolibrary.org/obo/GAZ_00068699"/>
        <obo:IAO_0000115>A wildlife refuge that is part of the Guanacaste Conservation Area and the Area de Conservacion Guanacaste World Heritage Site in the northwestern part of Costa Rica. It protects areas of tropical dry forest and coastal mangroves.</obo:IAO_0000115>
        <oboInOwl:hasOBONamespace>GAZ</oboInOwl:hasOBONamespace>
        <oboInOwl:id>GAZ:00068822</oboInOwl:id>
        <rdfs:label>Junquillal Bay Wildlife Refuge</rdfs:label>
    </owl:NamedIndividual>
    


    <!-- http://purl.obolibrary.org/obo/GAZ_00068823 -->

    <owl:NamedIndividual rdf:about="http://purl.obolibrary.org/obo/GAZ_00068823">
        <obo:RO_0001025 rdf:resource="http://purl.obolibrary.org/obo/GAZ_00068699"/>
        <obo:IAO_0000115>A national park, part of the Area de Conservacion Guanacaste World Heritage site, in the northern western part of Costa Rica, originally created to protect the scene of the Battle of Santa Rosa, at its eastern edge lies the Interamerican Highway where it is adjacent to the Guanacaste National Park, the main site is 36 km north of Liberia in Guanacaste Province. It was created in 1971.</obo:IAO_0000115>
        <oboInOwl:hasOBONamespace>GAZ</oboInOwl:hasOBONamespace>
        <oboInOwl:id>GAZ:00068823</oboInOwl:id>
        <rdfs:label>Parque Nacional Santa Rosa</rdfs:label>
    </owl:NamedIndividual>
    


    <!-- http://purl.obolibrary.org/obo/GAZ_00068824 -->

    <owl:NamedIndividual rdf:about="http://purl.obolibrary.org/obo/GAZ_00068824">
        <obo:RO_0001025 rdf:resource="http://purl.obolibrary.org/obo/GAZ_00003210"/>
        <obo:RO_0001025 rdf:resource="http://purl.obolibrary.org/obo/GAZ_00068699"/>
        <obo:IAO_0000115>A nature reserve which is part of the Guanacaste Conservation Area in northwestern Costa Rica. It is an experimental forest restoration program seeking to restore land previously converted to agriculture back to dry tropical forest.</obo:IAO_0000115>
        <oboInOwl:hasOBONamespace>GAZ</oboInOwl:hasOBONamespace>
        <oboInOwl:id>GAZ:00068824</oboInOwl:id>
        <rdfs:label>Horizontes Experimental Forest</rdfs:label>
    </owl:NamedIndividual>
    


    <!-- http://purl.obolibrary.org/obo/GAZ_00068825 -->

    <owl:NamedIndividual rdf:about="http://purl.obolibrary.org/obo/GAZ_00068825">
        <obo:RO_0001025 rdf:resource="http://purl.obolibrary.org/obo/GAZ_00003210"/>
        <obo:RO_0001025 rdf:resource="http://purl.obolibrary.org/obo/GAZ_00068699"/>
        <obo:IAO_0000115>A part of the Area de Conservacion Guanacaste World Heritage Site, is a National Park in the northern part of Costa Rica, from the slopes of the Orosi and Cacao volcanoes west to the Interamerican Highway where it is adjacent to the Santa Rosa National Park. It was created in 1989.</obo:IAO_0000115>
        <oboInOwl:hasOBONamespace>GAZ</oboInOwl:hasOBONamespace>
        <oboInOwl:id>GAZ:00068825</oboInOwl:id>
        <rdfs:label>Parque Nacional Guanacaste</rdfs:label>
    </owl:NamedIndividual>
    


    <!-- http://purl.obolibrary.org/obo/GAZ_00068826 -->

    <owl:NamedIndividual rdf:about="http://purl.obolibrary.org/obo/GAZ_00068826">
        <obo:RO_0001025 rdf:resource="http://purl.obolibrary.org/obo/GAZ_00002901"/>
        <obo:IAO_0000115>An administrative area which is managed by the Sistema Nacional de Areas de Conservacion for the purposes of conservation in the northern part of Costa Rica. It contains a National Park, and number of Wildlife refuges and Forest Reserves. It has been proposed that the Maquenque National Park be formed in this area, which would incorporate some of the existing nature reserves and expand on them.</obo:IAO_0000115>
        <oboInOwl:hasOBONamespace>GAZ</oboInOwl:hasOBONamespace>
        <oboInOwl:id>GAZ:00068826</oboInOwl:id>
        <rdfs:label>Arenal Huetar Norte Conservation Area</rdfs:label>
    </owl:NamedIndividual>
    


    <!-- http://purl.obolibrary.org/obo/GAZ_00068827 -->

    <owl:NamedIndividual rdf:about="http://purl.obolibrary.org/obo/GAZ_00068827">
        <rdf:type rdf:resource="http://purl.obolibrary.org/obo/ENVO_00000111"/>
        <obo:RO_0001025 rdf:resource="http://purl.obolibrary.org/obo/GAZ_00003205"/>
        <obo:RO_0001025 rdf:resource="http://purl.obolibrary.org/obo/GAZ_00068826"/>
        <obo:IAO_0000115>A Forest Reserve, part of the Arenal Huetar Norte Conservation Area, in the northern part of Costa Rica about 80 miles north of San Jose, to the north of nearby Boca Tapada and near the border with Nicaragua. There has been discussion of including this reserve as part of the proposed Maquenque National Park.</obo:IAO_0000115>
        <oboInOwl:hasOBONamespace>GAZ</oboInOwl:hasOBONamespace>
        <oboInOwl:id>GAZ:00068827</oboInOwl:id>
        <rdfs:label>Cerro El Jardin Forest Reserve</rdfs:label>
    </owl:NamedIndividual>
    


    <!-- http://purl.obolibrary.org/obo/GAZ_00068828 -->

    <owl:NamedIndividual rdf:about="http://purl.obolibrary.org/obo/GAZ_00068828">
        <obo:RO_0001025 rdf:resource="http://purl.obolibrary.org/obo/GAZ_00003205"/>
        <obo:RO_0001025 rdf:resource="http://purl.obolibrary.org/obo/GAZ_00068826"/>
        <obo:IAO_0000115>A wildlife refuge that is part of the Arenal Huetar Norte Conservation Area, in the northern part of Costa Rica, near Upala in the Alajuela Province, close to the border with Nicaragua.</obo:IAO_0000115>
        <oboInOwl:hasOBONamespace>GAZ</oboInOwl:hasOBONamespace>
        <oboInOwl:id>GAZ:00068828</oboInOwl:id>
        <rdfs:label>Laguna Las Camelias Wildlife Refuge</rdfs:label>
    </owl:NamedIndividual>
    


    <!-- http://purl.obolibrary.org/obo/GAZ_00068829 -->

    <owl:NamedIndividual rdf:about="http://purl.obolibrary.org/obo/GAZ_00068829">
        <obo:RO_0001025 rdf:resource="http://purl.obolibrary.org/obo/GAZ_00003208"/>
        <obo:RO_0001025 rdf:resource="http://purl.obolibrary.org/obo/GAZ_00068826"/>
        <obo:IAO_0000115>A nature reserve, part of the Arenal Huetar Norte Conservation Area, in the northern part of Costa Rica near the small town of Sardinal, Sarapiqui in the province of Heredia. It has been included as part of the proposed Maquenque National Park.</obo:IAO_0000115>
        <oboInOwl:hasOBONamespace>GAZ</oboInOwl:hasOBONamespace>
        <oboInOwl:id>GAZ:00068829</oboInOwl:id>
        <rdfs:label>Laguna Maquenque Wetlands</rdfs:label>
    </owl:NamedIndividual>
    


    <!-- http://purl.obolibrary.org/obo/GAZ_00068830 -->

    <owl:NamedIndividual rdf:about="http://purl.obolibrary.org/obo/GAZ_00068830">
        <obo:RO_0001025 rdf:resource="http://purl.obolibrary.org/obo/GAZ_00003205"/>
        <obo:RO_0001025 rdf:resource="http://purl.obolibrary.org/obo/GAZ_00068826"/>
        <obo:IAO_0000115>A national park, part of the Arenal Huetar Norte Conservation Area, in the northern part of Costa Rica about 100 km north of San Jose, to the east of Ciudad Quesada in Alajuela Province. It contains the active Platanar Volcano as well as the dormant Porvenir Volcano. It was created in 1992.</obo:IAO_0000115>
        <oboInOwl:hasOBONamespace>GAZ</oboInOwl:hasOBONamespace>
        <oboInOwl:id>GAZ:00068830</oboInOwl:id>
        <rdfs:label>Juan Castro Blanco National Park</rdfs:label>
    </owl:NamedIndividual>
    


    <!-- http://purl.obolibrary.org/obo/GAZ_00068831 -->

    <owl:NamedIndividual rdf:about="http://purl.obolibrary.org/obo/GAZ_00068831">
        <obo:RO_0001025 rdf:resource="http://purl.obolibrary.org/obo/GAZ_00003205"/>
        <obo:RO_0001025 rdf:resource="http://purl.obolibrary.org/obo/GAZ_00068826"/>
        <obo:IAO_0000115>A wildlife refuge, part of the Arenal Huetar Norte Conservation Area, in the northern part of Costa Rica twenty km south of Los Chiles near the border with Nicaragua in the Alajuela province.</obo:IAO_0000115>
        <oboInOwl:hasOBONamespace>GAZ</oboInOwl:hasOBONamespace>
        <oboInOwl:id>GAZ:00068831</oboInOwl:id>
        <rdfs:label>Cano Negro Wildlife Refuge</rdfs:label>
    </owl:NamedIndividual>
    


    <!-- http://purl.obolibrary.org/obo/GAZ_00068832 -->

    <owl:NamedIndividual rdf:about="http://purl.obolibrary.org/obo/GAZ_00068832">
        <obo:RO_0001025 rdf:resource="http://purl.obolibrary.org/obo/GAZ_00003208"/>
        <obo:RO_0001025 rdf:resource="http://purl.obolibrary.org/obo/GAZ_00068826"/>
        <obo:IAO_0000115>A nature reserve, part of the Arenal Huetar Norte Conservation Area, in the northern part of Costa Rica about 80 miles north of San Jose, to the east of Boca Tapada. It protects wetland forest areas near the border with Nicaragua, and is part of the proposed Maquenque National Park.</obo:IAO_0000115>
        <oboInOwl:hasOBONamespace>GAZ</oboInOwl:hasOBONamespace>
        <oboInOwl:id>GAZ:00068832</oboInOwl:id>
        <rdfs:label>Lacustrino de Tamborcito Wetlands</rdfs:label>
    </owl:NamedIndividual>
    


    <!-- http://purl.obolibrary.org/obo/GAZ_00068833 -->

    <owl:NamedIndividual rdf:about="http://purl.obolibrary.org/obo/GAZ_00068833">
        <obo:RO_0001025 rdf:resource="http://purl.obolibrary.org/obo/GAZ_00003208"/>
        <obo:RO_0001025 rdf:resource="http://purl.obolibrary.org/obo/GAZ_00068826"/>
        <obo:IAO_0000115>A part of the Arenal Huetar Norte Conservation Area, in the northern part of Costa Rica about 130 km north of San Jose, to the east of Boca Tapada. It was created in 1994 to poretect forests near the border with Nicaragua. It is included in proposals to create the new Maquenque National Park.</obo:IAO_0000115>
        <oboInOwl:hasOBONamespace>GAZ</oboInOwl:hasOBONamespace>
        <oboInOwl:id>GAZ:00068833</oboInOwl:id>
        <rdfs:label>La Curena Forest Reserve</rdfs:label>
    </owl:NamedIndividual>
    


    <!-- http://purl.obolibrary.org/obo/GAZ_00068834 -->

    <owl:NamedIndividual rdf:about="http://purl.obolibrary.org/obo/GAZ_00068834">
        <rdf:type rdf:resource="http://purl.obolibrary.org/obo/ENVO_00000111"/>
        <obo:RO_0001025 rdf:resource="http://purl.obolibrary.org/obo/GAZ_00003205"/>
        <obo:RO_0001025 rdf:resource="http://purl.obolibrary.org/obo/GAZ_00068826"/>
        <obo:IAO_0000115>A Forest Reserve, part of the Arenal Huetar Norte Conservation Area, in the northern part of Costa Rica in the emergency zone of the Arenal Volcano. It was created in 1972.</obo:IAO_0000115>
        <oboInOwl:hasOBONamespace>GAZ</oboInOwl:hasOBONamespace>
        <oboInOwl:id>GAZ:00068834</oboInOwl:id>
        <rdfs:label>Arenal Volcano Emergency Forest Reserve</rdfs:label>
    </owl:NamedIndividual>
    


    <!-- http://purl.obolibrary.org/obo/GAZ_00068835 -->

    <owl:NamedIndividual rdf:about="http://purl.obolibrary.org/obo/GAZ_00068835">
        <obo:RO_0001025 rdf:resource="http://purl.obolibrary.org/obo/GAZ_00002902"/>
        <obo:IAO_0000115>A World Heritage Site.</obo:IAO_0000115>
        <oboInOwl:hasOBONamespace>GAZ</oboInOwl:hasOBONamespace>
        <oboInOwl:id>GAZ:00068835</oboInOwl:id>
        <rdfs:label>Cocos Island National Park</rdfs:label>
    </owl:NamedIndividual>
    


    <!-- http://purl.obolibrary.org/obo/GAZ_00068836 -->

    <owl:NamedIndividual rdf:about="http://purl.obolibrary.org/obo/GAZ_00068836">
        <obo:RO_0001025 rdf:resource="http://purl.obolibrary.org/obo/GAZ_00002901"/>
        <obo:IAO_0000115>An administrative area which is managed by SINAC for the purposes of conservation in the northeastern part of Costa Rica. It contains a National Park, several Wildlife refuges and Protected Zones.</obo:IAO_0000115>
        <oboInOwl:hasOBONamespace>GAZ</oboInOwl:hasOBONamespace>
        <oboInOwl:id>GAZ:00068836</oboInOwl:id>
        <rdfs:label>Tortuguero Conservation Area</rdfs:label>
    </owl:NamedIndividual>
    


    <!-- http://purl.obolibrary.org/obo/GAZ_00068837 -->

    <owl:NamedIndividual rdf:about="http://purl.obolibrary.org/obo/GAZ_00068837">
        <obo:RO_0001025 rdf:resource="http://purl.obolibrary.org/obo/GAZ_00003206"/>
        <obo:RO_0001025 rdf:resource="http://purl.obolibrary.org/obo/GAZ_00068836"/>
        <obo:RO_0001025 rdf:resource="http://purl.obolibrary.org/obo/GAZ_00068879"/>
        <obo:IAO_0000115>A nature reserve, part of both the Tortuguero and Caribbean La Amistad Conservation Areas, in the Limon Province of northeastern Costa Rica. It covers all of the coast from the Tortuguero National Park to the Pacuare Matina Forest Reserve.</obo:IAO_0000115>
        <oboInOwl:hasOBONamespace>GAZ</oboInOwl:hasOBONamespace>
        <oboInOwl:id>GAZ:00068837</oboInOwl:id>
        <rdfs:label>Cariari National Wetlands</rdfs:label>
    </owl:NamedIndividual>
    


    <!-- http://purl.obolibrary.org/obo/GAZ_00068838 -->

    <owl:NamedIndividual rdf:about="http://purl.obolibrary.org/obo/GAZ_00068838">
        <obo:RO_0001025 rdf:resource="http://purl.obolibrary.org/obo/GAZ_00003206"/>
        <obo:RO_0001025 rdf:resource="http://purl.obolibrary.org/obo/GAZ_00068836"/>
        <obo:IAO_0000115>A nature reserve, part of the Tortuguero Conservation Area, in the Limon Province of northeastern Costa Rica, which protects the recharge area of the Guacimo and Pococi rivers.</obo:IAO_0000115>
        <oboInOwl:hasOBONamespace>GAZ</oboInOwl:hasOBONamespace>
        <oboInOwl:id>GAZ:00068838</oboInOwl:id>
        <rdfs:label>Acuiferos Guacimo y Pococi Protected Zone</rdfs:label>
    </owl:NamedIndividual>
    


    <!-- http://purl.obolibrary.org/obo/GAZ_00068839 -->

    <owl:NamedIndividual rdf:about="http://purl.obolibrary.org/obo/GAZ_00068839">
        <obo:RO_0001025 rdf:resource="http://purl.obolibrary.org/obo/GAZ_00068735"/>
        <obo:RO_0001025 rdf:resource="http://purl.obolibrary.org/obo/GAZ_00068781"/>
        <obo:IAO_0000115>A national park in the Central Pacific Conservation Area located near the Pacific coast of Costa Rica that protects tropical forest in the Puriscal Canton region of the Cordillera de Talamanca.</obo:IAO_0000115>
        <oboInOwl:hasOBONamespace>GAZ</oboInOwl:hasOBONamespace>
        <oboInOwl:id>GAZ:00068839</oboInOwl:id>
        <rdfs:label>La Cangreja National Park</rdfs:label>
    </owl:NamedIndividual>
    


    <!-- http://purl.obolibrary.org/obo/GAZ_00068840 -->

    <owl:NamedIndividual rdf:about="http://purl.obolibrary.org/obo/GAZ_00068840">
        <obo:RO_0001025 rdf:resource="http://purl.obolibrary.org/obo/GAZ_00003209"/>
        <obo:RO_0001025 rdf:resource="http://purl.obolibrary.org/obo/GAZ_00068735"/>
        <obo:IAO_0000115>A national park in the Central Pacific Conservation Area located near the Pacific coast of Costa Rica. Carara National Park was established on 1978-04-27. Carara lies about 30 miles west of the Costa Rican capital of San Jose and about 15 miles north of the beach town of Jaco. The park protects the river basin of the River Tarcoles, near Orotina.</obo:IAO_0000115>
        <oboInOwl:hasOBONamespace>GAZ</oboInOwl:hasOBONamespace>
        <oboInOwl:id>GAZ:00068840</oboInOwl:id>
        <rdfs:label>Carara National Park</rdfs:label>
    </owl:NamedIndividual>
    


    <!-- http://purl.obolibrary.org/obo/GAZ_00068841 -->

    <owl:NamedIndividual rdf:about="http://purl.obolibrary.org/obo/GAZ_00068841">
        <obo:RO_0001025 rdf:resource="http://purl.obolibrary.org/obo/GAZ_00003209"/>
        <obo:RO_0001025 rdf:resource="http://purl.obolibrary.org/obo/GAZ_00068735"/>
        <obo:IAO_0000115>An area that protects tropical forest on the Pacific Coast of Costa Rica, west of Carara National Park.</obo:IAO_0000115>
        <oboInOwl:hasOBONamespace>GAZ</oboInOwl:hasOBONamespace>
        <oboInOwl:id>GAZ:00068841</oboInOwl:id>
        <rdfs:label>Surtubal Wildlife Refuge</rdfs:label>
    </owl:NamedIndividual>
    


    <!-- http://purl.obolibrary.org/obo/GAZ_00068842 -->

    <owl:NamedIndividual rdf:about="http://purl.obolibrary.org/obo/GAZ_00068842">
        <obo:RO_0001025 rdf:resource="http://purl.obolibrary.org/obo/GAZ_00003209"/>
        <obo:RO_0001025 rdf:resource="http://purl.obolibrary.org/obo/GAZ_00068690"/>
        <obo:RO_0001025 rdf:resource="http://purl.obolibrary.org/obo/GAZ_00068735"/>
        <oboInOwl:hasOBONamespace>GAZ</oboInOwl:hasOBONamespace>
        <oboInOwl:id>GAZ:00068842</oboInOwl:id>
        <rdfs:label>San Lucas Island Wildlife Refuge</rdfs:label>
    </owl:NamedIndividual>
    


    <!-- http://purl.obolibrary.org/obo/GAZ_00068843 -->

    <owl:NamedIndividual rdf:about="http://purl.obolibrary.org/obo/GAZ_00068843">
        <obo:RO_0001025 rdf:resource="http://purl.obolibrary.org/obo/GAZ_00003209"/>
        <obo:RO_0001025 rdf:resource="http://purl.obolibrary.org/obo/GAZ_00068735"/>
        <obo:IAO_0000115>An area that protects forested and coastal mangrove areas on the Pacific Coast of Costa Rica, south of Puntarenas. It is located between the mouth of the Rio Jesus Maria (Las Flores Estuary) to the south, and the Caldera Bay to the north.</obo:IAO_0000115>
        <oboInOwl:hasOBONamespace>GAZ</oboInOwl:hasOBONamespace>
        <oboInOwl:id>GAZ:00068843</oboInOwl:id>
        <rdfs:label>Tivives Protected Zone</rdfs:label>
    </owl:NamedIndividual>
    


    <!-- http://purl.obolibrary.org/obo/GAZ_00068844 -->

    <owl:NamedIndividual rdf:about="http://purl.obolibrary.org/obo/GAZ_00068844">
        <obo:RO_0001025 rdf:resource="http://purl.obolibrary.org/obo/GAZ_00003207"/>
        <obo:RO_0001025 rdf:resource="http://purl.obolibrary.org/obo/GAZ_00068735"/>
        <obo:IAO_0000115>An area that protects tropical forest areas in the northern Talamanca Mountain Range of Costa Rica, between Atenas and Orotina.</obo:IAO_0000115>
        <oboInOwl:hasOBONamespace>GAZ</oboInOwl:hasOBONamespace>
        <oboInOwl:id>GAZ:00068844</oboInOwl:id>
        <rdfs:label>Cerro Chompipe Protected Zone</rdfs:label>
    </owl:NamedIndividual>
    


    <!-- http://purl.obolibrary.org/obo/GAZ_00068845 -->

    <owl:NamedIndividual rdf:about="http://purl.obolibrary.org/obo/GAZ_00068845">
        <obo:RO_0001025 rdf:resource="http://purl.obolibrary.org/obo/GAZ_00003210"/>
        <obo:RO_0001025 rdf:resource="http://purl.obolibrary.org/obo/GAZ_00068735"/>
        <obo:IAO_0000115>A protected area that protects the slopes of Cerro Caraigres in the northern Talamanca Mountains of the Central Valley of Costa Rica.</obo:IAO_0000115>
        <oboInOwl:hasOBONamespace>GAZ</oboInOwl:hasOBONamespace>
        <oboInOwl:id>GAZ:00068845</oboInOwl:id>
        <rdfs:label>Caraigres Protected Zone</rdfs:label>
    </owl:NamedIndividual>
    


    <!-- http://purl.obolibrary.org/obo/GAZ_00068846 -->

    <owl:NamedIndividual rdf:about="http://purl.obolibrary.org/obo/GAZ_00068846">
        <obo:RO_0001025 rdf:resource="http://purl.obolibrary.org/obo/GAZ_00003209"/>
        <obo:RO_0001025 rdf:resource="http://purl.obolibrary.org/obo/GAZ_00068735"/>
        <obo:IAO_0000115>An area that protects tropical forest areas bordering the north side of Carara National Park, on the Pacific Coast of Costa Rica.</obo:IAO_0000115>
        <oboInOwl:hasOBONamespace>GAZ</oboInOwl:hasOBONamespace>
        <oboInOwl:id>GAZ:00068846</oboInOwl:id>
        <rdfs:label>Finca Hacienda La Avellana Wildlife</rdfs:label>
    </owl:NamedIndividual>
    


    <!-- http://purl.obolibrary.org/obo/GAZ_00068847 -->

    <owl:NamedIndividual rdf:about="http://purl.obolibrary.org/obo/GAZ_00068847">
        <obo:RO_0001025 rdf:resource="http://purl.obolibrary.org/obo/GAZ_00003207"/>
        <obo:RO_0001025 rdf:resource="http://purl.obolibrary.org/obo/GAZ_00003209"/>
        <obo:RO_0001025 rdf:resource="http://purl.obolibrary.org/obo/GAZ_00068735"/>
        <obo:IAO_0000115>An area that protects forest habitats in the Talamanca Mountains south and west of the city of San Jose. Within Los Santos. Includes the Cerro Las Vueltas Biological Reserve and the Paramo Wildlife Refuge.</obo:IAO_0000115>
        <oboInOwl:hasOBONamespace>GAZ</oboInOwl:hasOBONamespace>
        <oboInOwl:id>GAZ:00068847</oboInOwl:id>
        <rdfs:label>Los Santos Forest Reserve</rdfs:label>
    </owl:NamedIndividual>
    


    <!-- http://purl.obolibrary.org/obo/GAZ_00068848 -->

    <owl:NamedIndividual rdf:about="http://purl.obolibrary.org/obo/GAZ_00068848">
        <obo:RO_0001025 rdf:resource="http://purl.obolibrary.org/obo/GAZ_00003209"/>
        <obo:RO_0001025 rdf:resource="http://purl.obolibrary.org/obo/GAZ_00068735"/>
        <obo:IAO_0000115>An area that protects a nesting beach of the Olive Ridley turtle. South of Jaco, on the Pacific Coast of Puntarenas, Costa Rica.</obo:IAO_0000115>
        <oboInOwl:hasOBONamespace>GAZ</oboInOwl:hasOBONamespace>
        <oboInOwl:id>GAZ:00068848</oboInOwl:id>
        <rdfs:label>Playa Hermosa Wildlife Refuge</rdfs:label>
    </owl:NamedIndividual>
    


    <!-- http://purl.obolibrary.org/obo/GAZ_00068849 -->

    <owl:NamedIndividual rdf:about="http://purl.obolibrary.org/obo/GAZ_00068849">
        <obo:RO_0001025 rdf:resource="http://purl.obolibrary.org/obo/GAZ_00003209"/>
        <obo:RO_0001025 rdf:resource="http://purl.obolibrary.org/obo/GAZ_00068735"/>
        <obo:IAO_0000115>A protected area.</obo:IAO_0000115>
        <oboInOwl:hasOBONamespace>GAZ</oboInOwl:hasOBONamespace>
        <oboInOwl:id>GAZ:00068849</oboInOwl:id>
        <rdfs:label>Puntarenas Estuary Wetlands</rdfs:label>
    </owl:NamedIndividual>
    


    <!-- http://purl.obolibrary.org/obo/GAZ_00068850 -->

    <owl:NamedIndividual rdf:about="http://purl.obolibrary.org/obo/GAZ_00068850">
        <obo:RO_0001025 rdf:resource="http://purl.obolibrary.org/obo/GAZ_00003209"/>
        <obo:RO_0001025 rdf:resource="http://purl.obolibrary.org/obo/GAZ_00068690"/>
        <obo:RO_0001025 rdf:resource="http://purl.obolibrary.org/obo/GAZ_00068735"/>
        <obo:IAO_0000115>An area that protects an island in the Gulf of Nicoya, Costa Rica.</obo:IAO_0000115>
        <oboInOwl:hasOBONamespace>GAZ</oboInOwl:hasOBONamespace>
        <oboInOwl:id>GAZ:00068850</oboInOwl:id>
        <rdfs:label>Pajaros Island Biological Reserve</rdfs:label>
    </owl:NamedIndividual>
    


    <!-- http://purl.obolibrary.org/obo/GAZ_00068851 -->

    <owl:NamedIndividual rdf:about="http://purl.obolibrary.org/obo/GAZ_00068851">
        <obo:RO_0001025 rdf:resource="http://purl.obolibrary.org/obo/GAZ_00003209"/>
        <obo:RO_0001025 rdf:resource="http://purl.obolibrary.org/obo/GAZ_00068735"/>
        <obo:IAO_0000115>An area that protects tropical forest areas on the Pacific Coast of Costa Rica.</obo:IAO_0000115>
        <oboInOwl:hasOBONamespace>GAZ</oboInOwl:hasOBONamespace>
        <oboInOwl:id>GAZ:00068851</oboInOwl:id>
        <rdfs:label>Portalon Wildlife Refuge</rdfs:label>
    </owl:NamedIndividual>
    


    <!-- http://purl.obolibrary.org/obo/GAZ_00068852 -->

    <owl:NamedIndividual rdf:about="http://purl.obolibrary.org/obo/GAZ_00068852">
        <obo:RO_0001025 rdf:resource="http://purl.obolibrary.org/obo/GAZ_00003207"/>
        <obo:RO_0001025 rdf:resource="http://purl.obolibrary.org/obo/GAZ_00068735"/>
        <obo:IAO_0000115>An area that protects tropical forest areas near the Pacific Coast of Costa Rica.</obo:IAO_0000115>
        <oboInOwl:hasOBONamespace>GAZ</oboInOwl:hasOBONamespace>
        <oboInOwl:id>GAZ:00068852</oboInOwl:id>
        <rdfs:label>Cacyra Wildlife Refuge</rdfs:label>
    </owl:NamedIndividual>
    


    <!-- http://purl.obolibrary.org/obo/GAZ_00068853 -->

    <owl:NamedIndividual rdf:about="http://purl.obolibrary.org/obo/GAZ_00068853">
        <obo:RO_0001025 rdf:resource="http://purl.obolibrary.org/obo/GAZ_00003207"/>
        <obo:RO_0001025 rdf:resource="http://purl.obolibrary.org/obo/GAZ_00068735"/>
        <obo:IAO_0000115>An area that protects tropical forest and beach areas on the Pacific Coast of Costa Rica.</obo:IAO_0000115>
        <oboInOwl:hasOBONamespace>GAZ</oboInOwl:hasOBONamespace>
        <oboInOwl:id>GAZ:00068853</oboInOwl:id>
        <rdfs:label>Punta Leona Wildlife Refuge</rdfs:label>
    </owl:NamedIndividual>
    


    <!-- http://purl.obolibrary.org/obo/GAZ_00068854 -->

    <owl:NamedIndividual rdf:about="http://purl.obolibrary.org/obo/GAZ_00068854">
        <obo:RO_0001025 rdf:resource="http://purl.obolibrary.org/obo/GAZ_00003207"/>
        <obo:RO_0001025 rdf:resource="http://purl.obolibrary.org/obo/GAZ_00068735"/>
        <obo:IAO_0000115>An area that protects tropical forest areas in the Talamanca Mountain Range of Costa Rica.</obo:IAO_0000115>
        <oboInOwl:hasOBONamespace>GAZ</oboInOwl:hasOBONamespace>
        <oboInOwl:id>GAZ:00068854</oboInOwl:id>
        <rdfs:label>Cataratas Cerro Redondo Wildlife Refuge</rdfs:label>
    </owl:NamedIndividual>
    


    <!-- http://purl.obolibrary.org/obo/GAZ_00068855 -->

    <owl:NamedIndividual rdf:about="http://purl.obolibrary.org/obo/GAZ_00068855">
        <obo:RO_0001025 rdf:resource="http://purl.obolibrary.org/obo/GAZ_00003210"/>
        <obo:RO_0001025 rdf:resource="http://purl.obolibrary.org/obo/GAZ_00068735"/>
        <obo:IAO_0000115>A protected area.</obo:IAO_0000115>
        <oboInOwl:hasOBONamespace>GAZ</oboInOwl:hasOBONamespace>
        <oboInOwl:id>GAZ:00068855</oboInOwl:id>
        <rdfs:label>Transilvania Wildlife Refuge</rdfs:label>
    </owl:NamedIndividual>
    


    <!-- http://purl.obolibrary.org/obo/GAZ_00068856 -->

    <owl:NamedIndividual rdf:about="http://purl.obolibrary.org/obo/GAZ_00068856">
        <obo:RO_0001025 rdf:resource="http://purl.obolibrary.org/obo/GAZ_00003205"/>
        <obo:RO_0001025 rdf:resource="http://purl.obolibrary.org/obo/GAZ_00003207"/>
        <obo:RO_0001025 rdf:resource="http://purl.obolibrary.org/obo/GAZ_00068735"/>
        <obo:IAO_0000115>A protected area.</obo:IAO_0000115>
        <oboInOwl:hasOBONamespace>GAZ</oboInOwl:hasOBONamespace>
        <oboInOwl:id>GAZ:00068856</oboInOwl:id>
        <rdfs:label>Montes de Oro Protected Zone</rdfs:label>
    </owl:NamedIndividual>
    


    <!-- http://purl.obolibrary.org/obo/GAZ_00068857 -->

    <owl:NamedIndividual rdf:about="http://purl.obolibrary.org/obo/GAZ_00068857">
        <obo:RO_0001025 rdf:resource="http://purl.obolibrary.org/obo/GAZ_00068735"/>
        <oboInOwl:hasOBONamespace>GAZ</oboInOwl:hasOBONamespace>
        <oboInOwl:id>GAZ:00068857</oboInOwl:id>
        <rdfs:label>Playa Blanca Marine Wetlands</rdfs:label>
    </owl:NamedIndividual>
    


    <!-- http://purl.obolibrary.org/obo/GAZ_00068858 -->

    <owl:NamedIndividual rdf:about="http://purl.obolibrary.org/obo/GAZ_00068858">
        <obo:RO_0001025 rdf:resource="http://purl.obolibrary.org/obo/GAZ_00003207"/>
        <obo:RO_0001025 rdf:resource="http://purl.obolibrary.org/obo/GAZ_00068735"/>
        <obo:IAO_0000115>An area that protects tropical forest areas on the Pacific Coast of Costa Rica.</obo:IAO_0000115>
        <oboInOwl:hasOBONamespace>GAZ</oboInOwl:hasOBONamespace>
        <oboInOwl:id>GAZ:00068858</oboInOwl:id>
        <rdfs:label>Cerro Nara Protected Zone</rdfs:label>
    </owl:NamedIndividual>
    


    <!-- http://purl.obolibrary.org/obo/GAZ_00068859 -->

    <owl:NamedIndividual rdf:about="http://purl.obolibrary.org/obo/GAZ_00068859">
        <obo:RO_0001025 rdf:resource="http://purl.obolibrary.org/obo/GAZ_00068735"/>
        <obo:RO_0001025 rdf:resource="http://purl.obolibrary.org/obo/GAZ_00068847"/>
        <obo:IAO_0000115>An area that protects tropical forest areas in the high elevations of the Talamanca Mountains, Costa Rica.</obo:IAO_0000115>
        <oboInOwl:hasOBONamespace>GAZ</oboInOwl:hasOBONamespace>
        <oboInOwl:id>GAZ:00068859</oboInOwl:id>
        <rdfs:label>Paramo Wildlife Refuge</rdfs:label>
    </owl:NamedIndividual>
    


    <!-- http://purl.obolibrary.org/obo/GAZ_00068860 -->

    <owl:NamedIndividual rdf:about="http://purl.obolibrary.org/obo/GAZ_00068860">
        <obo:RO_0001025 rdf:resource="http://purl.obolibrary.org/obo/GAZ_00068735"/>
        <obo:RO_0001025 rdf:resource="http://purl.obolibrary.org/obo/GAZ_00068847"/>
        <obo:IAO_0000115>A protected area within the Los Santos Forest Reserve near the Pacific Coast of Costa Rica.</obo:IAO_0000115>
        <oboInOwl:hasOBONamespace>GAZ</oboInOwl:hasOBONamespace>
        <oboInOwl:id>GAZ:00068860</oboInOwl:id>
        <rdfs:label>Cerro las Vueltas Biological Reserve</rdfs:label>
    </owl:NamedIndividual>
    


    <!-- http://purl.obolibrary.org/obo/GAZ_00068861 -->

    <owl:NamedIndividual rdf:about="http://purl.obolibrary.org/obo/GAZ_00068861">
        <obo:RO_0001025 rdf:resource="http://purl.obolibrary.org/obo/GAZ_00003207"/>
        <obo:RO_0001025 rdf:resource="http://purl.obolibrary.org/obo/GAZ_00068735"/>
        <obo:RO_0001025 rdf:resource="http://purl.obolibrary.org/obo/GAZ_00068738"/>
        <obo:IAO_0000115>An area that protects tropical evergreen forest areas on the southern slopes of the Tilaran Mountains of Costa Rica. Site of the Penas Blancas River Hydroelectric Project. It is located within the Montes de Oro Protected Zone.</obo:IAO_0000115>
        <oboInOwl:hasOBONamespace>GAZ</oboInOwl:hasOBONamespace>
        <oboInOwl:id>GAZ:00068861</oboInOwl:id>
        <rdfs:label>Penas Blancas Wildlife Refuge</rdfs:label>
    </owl:NamedIndividual>
    


    <!-- http://purl.obolibrary.org/obo/GAZ_00068862 -->

    <owl:NamedIndividual rdf:about="http://purl.obolibrary.org/obo/GAZ_00068862">
        <obo:RO_0001025 rdf:resource="http://purl.obolibrary.org/obo/GAZ_00068735"/>
        <obo:RO_0001025 rdf:resource="http://purl.obolibrary.org/obo/GAZ_00068795"/>
        <obo:IAO_0000115>An area that protects tropical forest areas in the Central Valley of Costa Rica.</obo:IAO_0000115>
        <oboInOwl:hasOBONamespace>GAZ</oboInOwl:hasOBONamespace>
        <oboInOwl:id>GAZ:00068862</oboInOwl:id>
        <rdfs:label>Cerros de Escazu Protected Zone</rdfs:label>
    </owl:NamedIndividual>
    


    <!-- http://purl.obolibrary.org/obo/GAZ_00068863 -->

    <owl:NamedIndividual rdf:about="http://purl.obolibrary.org/obo/GAZ_00068863">
        <obo:RO_0001025 rdf:resource="http://purl.obolibrary.org/obo/GAZ_00003209"/>
        <obo:RO_0001025 rdf:resource="http://purl.obolibrary.org/obo/GAZ_00068735"/>
        <obo:IAO_0000115>A protected area.</obo:IAO_0000115>
        <oboInOwl:hasOBONamespace>GAZ</oboInOwl:hasOBONamespace>
        <oboInOwl:id>GAZ:00068863</oboInOwl:id>
        <rdfs:label>Cerros de Turrubares Protected Zone</rdfs:label>
    </owl:NamedIndividual>
    


    <!-- http://purl.obolibrary.org/obo/GAZ_00068864 -->

    <owl:NamedIndividual rdf:about="http://purl.obolibrary.org/obo/GAZ_00068864">
        <obo:RO_0001025 rdf:resource="http://purl.obolibrary.org/obo/GAZ_00003207"/>
        <obo:RO_0001025 rdf:resource="http://purl.obolibrary.org/obo/GAZ_00068735"/>
        <obo:IAO_0000115>An area that protects tropical forest areas, on the southeast border of Carara National Park Costa Rica.</obo:IAO_0000115>
        <oboInOwl:hasOBONamespace>GAZ</oboInOwl:hasOBONamespace>
        <oboInOwl:id>GAZ:00068864</oboInOwl:id>
        <rdfs:label>Fernando Castro Cervantes Wildlife</rdfs:label>
    </owl:NamedIndividual>
    


    <!-- http://purl.obolibrary.org/obo/GAZ_00068865 -->

    <owl:NamedIndividual rdf:about="http://purl.obolibrary.org/obo/GAZ_00068865">
        <obo:RO_0001025 rdf:resource="http://purl.obolibrary.org/obo/GAZ_00003207"/>
        <obo:RO_0001025 rdf:resource="http://purl.obolibrary.org/obo/GAZ_00068735"/>
        <obo:IAO_0000115>An area that protects tropical forest areas in the Central Valley area of Costa Rica.</obo:IAO_0000115>
        <oboInOwl:hasOBONamespace>GAZ</oboInOwl:hasOBONamespace>
        <oboInOwl:id>GAZ:00068865</oboInOwl:id>
        <rdfs:label>Quitirrisi Protected Zone</rdfs:label>
    </owl:NamedIndividual>
    


    <!-- http://purl.obolibrary.org/obo/GAZ_00068866 -->

    <owl:NamedIndividual rdf:about="http://purl.obolibrary.org/obo/GAZ_00068866">
        <obo:RO_0001025 rdf:resource="http://purl.obolibrary.org/obo/GAZ_00003207"/>
        <obo:RO_0001025 rdf:resource="http://purl.obolibrary.org/obo/GAZ_00068735"/>
        <obo:IAO_0000115>An area that protects tropical forest areas northwest of Cerros de Escazu and Quitirrisi, Costa Rica.</obo:IAO_0000115>
        <oboInOwl:hasOBONamespace>GAZ</oboInOwl:hasOBONamespace>
        <oboInOwl:id>GAZ:00068866</oboInOwl:id>
        <rdfs:label>El Rodeo Protected Zone</rdfs:label>
    </owl:NamedIndividual>
    


    <!-- http://purl.obolibrary.org/obo/GAZ_00068867 -->

    <owl:NamedIndividual rdf:about="http://purl.obolibrary.org/obo/GAZ_00068867">
        <obo:RO_0001025 rdf:resource="http://purl.obolibrary.org/obo/GAZ_00003209"/>
        <obo:RO_0001025 rdf:resource="http://purl.obolibrary.org/obo/GAZ_00068735"/>
        <obo:IAO_0000115>An area that protects mangroves and wetlands at the mouth of the Rio Abangares, which empties into the Gulf of Nicoya north of Pajaros Island.</obo:IAO_0000115>
        <oboInOwl:hasOBONamespace>GAZ</oboInOwl:hasOBONamespace>
        <oboInOwl:id>GAZ:00068867</oboInOwl:id>
        <rdfs:label>La Ensenada Wildlife Refuge</rdfs:label>
    </owl:NamedIndividual>
    


    <!-- http://purl.obolibrary.org/obo/GAZ_00068868 -->

    <owl:NamedIndividual rdf:about="http://purl.obolibrary.org/obo/GAZ_00068868">
        <obo:RO_0001025 rdf:resource="http://purl.obolibrary.org/obo/GAZ_00003209"/>
        <obo:RO_0001025 rdf:resource="http://purl.obolibrary.org/obo/GAZ_00068735"/>
        <obo:IAO_0000115>An area that protects tropical forest areas on the Pacific Coast, near Dominical, Aguirre Costa Rica.</obo:IAO_0000115>
        <oboInOwl:hasOBONamespace>GAZ</oboInOwl:hasOBONamespace>
        <oboInOwl:id>GAZ:00068868</oboInOwl:id>
        <rdfs:label>Finca Baru Pacifico Wildlife Refuge</rdfs:label>
    </owl:NamedIndividual>
    


    <!-- http://purl.obolibrary.org/obo/GAZ_00068869 -->

    <owl:NamedIndividual rdf:about="http://purl.obolibrary.org/obo/GAZ_00068869">
        <obo:RO_0001025 rdf:resource="http://purl.obolibrary.org/obo/GAZ_00002901"/>
        <obo:IAO_0000115>An administrative area which is managed by the Sistema Nacional de Areas de Conservacion for the purposes of conservation in the southern part of Costa Rica, on the Pacific side of the Continental Divide. It contains several National Parks, and a number Wildlife refuges and other types of nature reserve.</obo:IAO_0000115>
        <oboInOwl:hasOBONamespace>GAZ</oboInOwl:hasOBONamespace>
        <oboInOwl:id>GAZ:00068869</oboInOwl:id>
        <rdfs:label>Pacific La Amistad Conservation Area</rdfs:label>
    </owl:NamedIndividual>
    


    <!-- http://purl.obolibrary.org/obo/GAZ_00068870 -->

    <owl:NamedIndividual rdf:about="http://purl.obolibrary.org/obo/GAZ_00068870">
        <obo:RO_0001025 rdf:resource="http://purl.obolibrary.org/obo/GAZ_00003207"/>
        <obo:RO_0001025 rdf:resource="http://purl.obolibrary.org/obo/GAZ_00068869"/>
        <obo:IAO_0000115>An area that protects forested areas in the southern Talamanca Mountain region near Tapanti National Park and Chirripo National Park. It is part of the La Amistad Biosphere designated by UNESCO.</obo:IAO_0000115>
        <oboInOwl:hasOBONamespace>GAZ</oboInOwl:hasOBONamespace>
        <oboInOwl:id>GAZ:00068870</oboInOwl:id>
        <rdfs:label>Rio Macho Forest Reserve</rdfs:label>
    </owl:NamedIndividual>
    


    <!-- http://purl.obolibrary.org/obo/GAZ_00068871 -->

    <owl:NamedIndividual rdf:about="http://purl.obolibrary.org/obo/GAZ_00068871">
        <obo:RO_0001025 rdf:resource="http://purl.obolibrary.org/obo/GAZ_00003209"/>
        <obo:RO_0001025 rdf:resource="http://purl.obolibrary.org/obo/GAZ_00068869"/>
        <obo:IAO_0000115>An area tha protects lowland areas in the foothills of the southern Talamanca Mountain region. These wetlands are east of the town of San Vito de Coto Brus.</obo:IAO_0000115>
        <oboInOwl:hasOBONamespace>GAZ</oboInOwl:hasOBONamespace>
        <oboInOwl:id>GAZ:00068871</oboInOwl:id>
        <rdfs:label>San Vito Wetlands</rdfs:label>
    </owl:NamedIndividual>
    


    <!-- http://purl.obolibrary.org/obo/GAZ_00068872 -->

    <owl:NamedIndividual rdf:about="http://purl.obolibrary.org/obo/GAZ_00068872">
        <obo:RO_0001025 rdf:resource="http://purl.obolibrary.org/obo/GAZ_00003210"/>
        <obo:RO_0001025 rdf:resource="http://purl.obolibrary.org/obo/GAZ_00068869"/>
        <obo:IAO_0000115>An area that protects lowland areas in the foothills of the southern Talamanca Mountain region. The lake is just south of the Wilson Botanical Gardens near San Vito de Coto Brus.</obo:IAO_0000115>
        <oboInOwl:hasOBONamespace>GAZ</oboInOwl:hasOBONamespace>
        <oboInOwl:id>GAZ:00068872</oboInOwl:id>
        <rdfs:label>Palustrino Laguna del Paraguas Wetlands</rdfs:label>
    </owl:NamedIndividual>
    


    <!-- http://purl.obolibrary.org/obo/GAZ_00068873 -->

    <owl:NamedIndividual rdf:about="http://purl.obolibrary.org/obo/GAZ_00068873">
        <obo:RO_0001025 rdf:resource="http://purl.obolibrary.org/obo/GAZ_00003207"/>
        <obo:RO_0001025 rdf:resource="http://purl.obolibrary.org/obo/GAZ_00068869"/>
        <obo:IAO_0000115>An area that protects forested areas in the Talamanca Mountain region, between the Los Santos Forest Reserve and Tapanti National Park.</obo:IAO_0000115>
        <oboInOwl:hasOBONamespace>GAZ</oboInOwl:hasOBONamespace>
        <oboInOwl:id>GAZ:00068873</oboInOwl:id>
        <rdfs:label>Joseph Steve Friedman Wildlife Refuge</rdfs:label>
    </owl:NamedIndividual>
    


    <!-- http://purl.obolibrary.org/obo/GAZ_00068874 -->

    <owl:NamedIndividual rdf:about="http://purl.obolibrary.org/obo/GAZ_00068874">
        <obo:RO_0001025 rdf:resource="http://purl.obolibrary.org/obo/GAZ_00003212"/>
        <obo:RO_0001025 rdf:resource="http://purl.obolibrary.org/obo/GAZ_00068869"/>
        <obo:IAO_0000115>A protected area that is a southern extension of La Amistad National Park, and part of the La Amistad Biosphere declared by UNESCO. It protects the southern portion of the country bordering on Panama.</obo:IAO_0000115>
        <oboInOwl:hasOBONamespace>GAZ</oboInOwl:hasOBONamespace>
        <oboInOwl:id>GAZ:00068874</oboInOwl:id>
        <rdfs:label>Las Tablas Protected Zone</rdfs:label>
    </owl:NamedIndividual>
    


    <!-- http://purl.obolibrary.org/obo/GAZ_00068875 -->

    <owl:NamedIndividual rdf:about="http://purl.obolibrary.org/obo/GAZ_00068875">
        <obo:RO_0001025 rdf:resource="http://purl.obolibrary.org/obo/GAZ_00003207"/>
        <obo:RO_0001025 rdf:resource="http://purl.obolibrary.org/obo/GAZ_00068869"/>
        <obo:IAO_0000115>An area that protects the Navarro and Sombrero River Basins.</obo:IAO_0000115>
        <oboInOwl:hasOBONamespace>GAZ</oboInOwl:hasOBONamespace>
        <oboInOwl:id>GAZ:00068875</oboInOwl:id>
        <rdfs:label>Rio Navarro-Rio Sombrero Protected Zone</rdfs:label>
    </owl:NamedIndividual>
    


    <!-- http://purl.obolibrary.org/obo/GAZ_00068876 -->

    <owl:NamedIndividual rdf:about="http://purl.obolibrary.org/obo/GAZ_00068876">
        <obo:RO_0001025 rdf:resource="http://purl.obolibrary.org/obo/GAZ_00003206"/>
        <obo:RO_0001025 rdf:resource="http://purl.obolibrary.org/obo/GAZ_00003207"/>
        <obo:RO_0001025 rdf:resource="http://purl.obolibrary.org/obo/GAZ_00003209"/>
        <obo:RO_0001025 rdf:resource="http://purl.obolibrary.org/obo/GAZ_00068869"/>
        <obo:RO_0001025 rdf:resource="http://purl.obolibrary.org/obo/GAZ_00068879"/>
        <obo:IAO_0000115>An international peace park in Latin America, management of which is shared between Costa Rica (Caribbean La Amistad and Pacific La Amistad Conservation Areas) and Panama, following a recommendation by UNESCO after the park&apos;s inclusion in the World Heritage Site list. The majority of the park area is in Costa Rica, as part of the former La Amistad Reserves of the Talamanca mountain range.</obo:IAO_0000115>
        <oboInOwl:hasOBONamespace>GAZ</oboInOwl:hasOBONamespace>
        <oboInOwl:id>GAZ:00068876</oboInOwl:id>
        <rdfs:label>Parque Internacional La Amistad</rdfs:label>
    </owl:NamedIndividual>
    


    <!-- http://purl.obolibrary.org/obo/GAZ_00068877 -->

    <owl:NamedIndividual rdf:about="http://purl.obolibrary.org/obo/GAZ_00068877">
        <obo:RO_0001025 rdf:resource="http://purl.obolibrary.org/obo/GAZ_00003211"/>
        <obo:RO_0001025 rdf:resource="http://purl.obolibrary.org/obo/GAZ_00068869"/>
        <obo:IAO_0000115>A national park in the Pacific La Amistad Conservation Area of Costa Rica located on the edge of the Talamanca Range, near Cartago. It protects forests to the north of Chirripo National Park, and also contains part of the Orosi River.</obo:IAO_0000115>
        <oboInOwl:hasOBONamespace>GAZ</oboInOwl:hasOBONamespace>
        <oboInOwl:id>GAZ:00068877</oboInOwl:id>
        <rdfs:label>Tapanti National Park</rdfs:label>
    </owl:NamedIndividual>
    


    <!-- http://purl.obolibrary.org/obo/GAZ_00068878 -->

    <owl:NamedIndividual rdf:about="http://purl.obolibrary.org/obo/GAZ_00068878">
        <obo:RO_0001025 rdf:resource="http://purl.obolibrary.org/obo/GAZ_00003206"/>
        <obo:RO_0001025 rdf:resource="http://purl.obolibrary.org/obo/GAZ_00003207"/>
        <obo:RO_0001025 rdf:resource="http://purl.obolibrary.org/obo/GAZ_00003211"/>
        <obo:RO_0001025 rdf:resource="http://purl.obolibrary.org/obo/GAZ_00068869"/>
        <obo:IAO_0000115>A national park in the Pacific La Amistad Conservation Area located in the Cordillera de Talamanca of Costa Rica that contains Cerro Chirripo, the highest mountain in the country at 3820 m. It covers parts of three Provinces in Costa Rica - San Jose, Limon and Cartago.</obo:IAO_0000115>
        <oboInOwl:hasOBONamespace>GAZ</oboInOwl:hasOBONamespace>
        <oboInOwl:id>GAZ:00068878</oboInOwl:id>
        <rdfs:label>Parque Nacional Chirripo</rdfs:label>
    </owl:NamedIndividual>
    


    <!-- http://purl.obolibrary.org/obo/GAZ_00068879 -->

    <owl:NamedIndividual rdf:about="http://purl.obolibrary.org/obo/GAZ_00068879">
        <obo:RO_0001025 rdf:resource="http://purl.obolibrary.org/obo/GAZ_00002901"/>
        <obo:IAO_0000115>An administrative area which is managed by the Sistema Nacional de Areas de Conservacion, for the purposes of conservation in the eastern part of Costa Rica, on the Caribbean coast. It contains several National Parks, and a number Wildlife refuges and other types of nature reserve.</obo:IAO_0000115>
        <oboInOwl:hasOBONamespace>GAZ</oboInOwl:hasOBONamespace>
        <oboInOwl:id>GAZ:00068879</oboInOwl:id>
        <rdfs:label>Caribbean La Amistad Conservation Area</rdfs:label>
    </owl:NamedIndividual>
    


    <!-- http://purl.obolibrary.org/obo/GAZ_00068880 -->

    <owl:NamedIndividual rdf:about="http://purl.obolibrary.org/obo/GAZ_00068880">
        <obo:RO_0001025 rdf:resource="http://purl.obolibrary.org/obo/GAZ_00003206"/>
        <obo:RO_0001025 rdf:resource="http://purl.obolibrary.org/obo/GAZ_00068879"/>
        <obo:IAO_0000115>A national park in the Caribbean La Amistad Conservation Area of Costa Rica located on the southern Caribbean coast in Limon Province, connected to the town of Cahuita.</obo:IAO_0000115>
        <oboInOwl:hasOBONamespace>GAZ</oboInOwl:hasOBONamespace>
        <oboInOwl:id>GAZ:00068880</oboInOwl:id>
        <rdfs:label>Cahuita National Park</rdfs:label>
    </owl:NamedIndividual>
    


    <!-- http://purl.obolibrary.org/obo/GAZ_00068881 -->

    <owl:NamedIndividual rdf:about="http://purl.obolibrary.org/obo/GAZ_00068881">
        <obo:RO_0001025 rdf:resource="http://purl.obolibrary.org/obo/GAZ_00003206"/>
        <obo:RO_0001025 rdf:resource="http://purl.obolibrary.org/obo/GAZ_00003211"/>
        <obo:RO_0001025 rdf:resource="http://purl.obolibrary.org/obo/GAZ_00068879"/>
        <obo:IAO_0000115>A national park in the Caribbean La Amistad Conservation Area of Costa Rica located on the eastern slopes of the Cordillera de Talamanca. It protects forests as well as Laguna Ayil and Cerro Tigre and the Dantas River watershed, covering parts of both Cartago and Limon Provinces.</obo:IAO_0000115>
        <oboInOwl:hasOBONamespace>GAZ</oboInOwl:hasOBONamespace>
        <oboInOwl:id>GAZ:00068881</oboInOwl:id>
        <rdfs:label>Barbilla National Park</rdfs:label>
    </owl:NamedIndividual>
    


    <!-- http://purl.obolibrary.org/obo/GAZ_00068882 -->

    <owl:NamedIndividual rdf:about="http://purl.obolibrary.org/obo/GAZ_00068882">
        <obo:RO_0001025 rdf:resource="http://purl.obolibrary.org/obo/GAZ_00003211"/>
        <obo:RO_0001025 rdf:resource="http://purl.obolibrary.org/obo/GAZ_00068879"/>
        <obo:IAO_0000115>An area that protects a lake on the eastern slope of the Talamanca Mountain Range of Costa Rica. Near Perralta, Turrialba, Cartago Province.</obo:IAO_0000115>
        <oboInOwl:hasOBONamespace>GAZ</oboInOwl:hasOBONamespace>
        <oboInOwl:id>GAZ:00068882</oboInOwl:id>
        <rdfs:label>Lacustrino Bonilla-Bonillita Wetlands</rdfs:label>
    </owl:NamedIndividual>
    


    <!-- http://purl.obolibrary.org/obo/GAZ_00068883 -->

    <owl:NamedIndividual rdf:about="http://purl.obolibrary.org/obo/GAZ_00068883">
        <obo:RO_0001025 rdf:resource="http://purl.obolibrary.org/obo/GAZ_00003211"/>
        <obo:RO_0001025 rdf:resource="http://purl.obolibrary.org/obo/GAZ_00068879"/>
        <obo:IAO_0000115>An area that protects forests and river basins of the Talamanca Mountain Range on the Caribbean slopes.</obo:IAO_0000115>
        <oboInOwl:hasOBONamespace>GAZ</oboInOwl:hasOBONamespace>
        <oboInOwl:id>GAZ:00068883</oboInOwl:id>
        <rdfs:label>Rio Pacuare Forest Reserve</rdfs:label>
    </owl:NamedIndividual>
    


    <!-- http://purl.obolibrary.org/obo/GAZ_00068884 -->

    <owl:NamedIndividual rdf:about="http://purl.obolibrary.org/obo/GAZ_00068884">
        <obo:RO_0001025 rdf:resource="http://purl.obolibrary.org/obo/GAZ_00003206"/>
        <obo:RO_0001025 rdf:resource="http://purl.obolibrary.org/obo/GAZ_00003211"/>
        <obo:RO_0001025 rdf:resource="http://purl.obolibrary.org/obo/GAZ_00068879"/>
        <obo:IAO_0000115>A protected area that covers the Siquirres River Basin near Bonilla. Costa Rica.</obo:IAO_0000115>
        <oboInOwl:hasOBONamespace>GAZ</oboInOwl:hasOBONamespace>
        <oboInOwl:id>GAZ:00068884</oboInOwl:id>
        <rdfs:label>Cuenca Rio Siquirres Protected Zone</rdfs:label>
    </owl:NamedIndividual>
    


    <!-- http://purl.obolibrary.org/obo/GAZ_00068885 -->

    <owl:NamedIndividual rdf:about="http://purl.obolibrary.org/obo/GAZ_00068885">
        <obo:RO_0001025 rdf:resource="http://purl.obolibrary.org/obo/GAZ_00068721"/>
        <obo:RO_0001025 rdf:resource="http://purl.obolibrary.org/obo/GAZ_00068879"/>
        <obo:IAO_0000115>An area that protects the lowlands of the southern Caribbean coastal region of Costa Rica. This coastal zone is between the mouths of the Rio Cocles and the Rio Sixaola, which forms the border with Panama. The refuge also protects a coral reef front across Punta Uva, Manzanillo and Uva.</obo:IAO_0000115>
        <oboInOwl:hasOBONamespace>GAZ</oboInOwl:hasOBONamespace>
        <oboInOwl:id>GAZ:00068885</oboInOwl:id>
        <rdfs:label>Gandoca Manzanillo Wildlife Refuge</rdfs:label>
    </owl:NamedIndividual>
    


    <!-- http://purl.obolibrary.org/obo/GAZ_00068886 -->

    <owl:NamedIndividual rdf:about="http://purl.obolibrary.org/obo/GAZ_00068886">
        <obo:RO_0001025 rdf:resource="http://purl.obolibrary.org/obo/GAZ_00003206"/>
        <obo:RO_0001025 rdf:resource="http://purl.obolibrary.org/obo/GAZ_00068879"/>
        <obo:IAO_0000115>An area that protects the lowland forests of the central Caribbean coastal region. This area includes the Madre de Dios Estuary at the mouth of the Pacuare River.</obo:IAO_0000115>
        <oboInOwl:hasOBONamespace>GAZ</oboInOwl:hasOBONamespace>
        <oboInOwl:id>GAZ:00068886</oboInOwl:id>
        <rdfs:label>Pacuare Matina Forest Reserve</rdfs:label>
    </owl:NamedIndividual>
    


    <!-- http://purl.obolibrary.org/obo/GAZ_00068887 -->

    <owl:NamedIndividual rdf:about="http://purl.obolibrary.org/obo/GAZ_00068887">
        <obo:RO_0001025 rdf:resource="http://purl.obolibrary.org/obo/GAZ_00068721"/>
        <obo:RO_0001025 rdf:resource="http://purl.obolibrary.org/obo/GAZ_00068879"/>
        <obo:IAO_0000115>An area that protects the foothills of the Talamanca Mountain Range in the Caribbean Brunca region. The primary river basins are the Rio Hitoy and the Rio Cerere.</obo:IAO_0000115>
        <oboInOwl:hasOBONamespace>GAZ</oboInOwl:hasOBONamespace>
        <oboInOwl:id>GAZ:00068887</oboInOwl:id>
        <rdfs:label>Hitoy Cerere Biological Reserve</rdfs:label>
    </owl:NamedIndividual>
    


    <!-- http://purl.obolibrary.org/obo/GAZ_00068888 -->

    <owl:NamedIndividual rdf:about="http://purl.obolibrary.org/obo/GAZ_00068888">
        <obo:RO_0001025 rdf:resource="http://purl.obolibrary.org/obo/GAZ_00003206"/>
        <obo:RO_0001025 rdf:resource="http://purl.obolibrary.org/obo/GAZ_00068879"/>
        <obo:IAO_0000115>A protected area.</obo:IAO_0000115>
        <oboInOwl:hasOBONamespace>GAZ</oboInOwl:hasOBONamespace>
        <oboInOwl:id>GAZ:00068888</oboInOwl:id>
        <rdfs:label>Aviarios del Caribe Wildlife Refuge</rdfs:label>
    </owl:NamedIndividual>
    


    <!-- http://purl.obolibrary.org/obo/GAZ_00068889 -->

    <owl:NamedIndividual rdf:about="http://purl.obolibrary.org/obo/GAZ_00068889">
        <obo:RO_0001025 rdf:resource="http://purl.obolibrary.org/obo/GAZ_00003206"/>
        <obo:RO_0001025 rdf:resource="http://purl.obolibrary.org/obo/GAZ_00068879"/>
        <obo:IAO_0000115>An area that protects the Banano River Basin, near Limoncito, north of the La Amistad International Park.</obo:IAO_0000115>
        <oboInOwl:hasOBONamespace>GAZ</oboInOwl:hasOBONamespace>
        <oboInOwl:id>GAZ:00068889</oboInOwl:id>
        <rdfs:label>Cuenca Rio Banano Protected Zone</rdfs:label>
    </owl:NamedIndividual>
    


    <!-- http://purl.obolibrary.org/obo/GAZ_00068890 -->

    <owl:NamedIndividual rdf:about="http://purl.obolibrary.org/obo/GAZ_00068890">
        <obo:RO_0001025 rdf:resource="http://purl.obolibrary.org/obo/GAZ_00003206"/>
        <obo:RO_0001025 rdf:resource="http://purl.obolibrary.org/obo/GAZ_00068879"/>
        <obo:IAO_0000115>A protected area located at the mouth of the Rio Limoncito, just south of the port city of Limon, Costa Rica.</obo:IAO_0000115>
        <oboInOwl:hasOBONamespace>GAZ</oboInOwl:hasOBONamespace>
        <oboInOwl:id>GAZ:00068890</oboInOwl:id>
        <rdfs:label>Limoncito Wildlife Refuge</rdfs:label>
    </owl:NamedIndividual>
    


    <!-- http://purl.obolibrary.org/obo/GAZ_00068891 -->

    <owl:NamedIndividual rdf:about="http://purl.obolibrary.org/obo/GAZ_00068891">
        <obo:RO_0001025 rdf:resource="http://purl.obolibrary.org/obo/GAZ_00002901"/>
        <obo:IAO_0000115>An administrative area which is managed by the Sistema Nacional de Areas de Conservacion for the purposes of conservation in the central part of Costa Rica, near the Arenal Volcano and covering the Cordillera de Tilaran. It contains a number of National Parks, Wildlife refuges and Protected Zones.</obo:IAO_0000115>
        <oboInOwl:hasOBONamespace>GAZ</oboInOwl:hasOBONamespace>
        <oboInOwl:id>GAZ:00068891</oboInOwl:id>
        <rdfs:label>Arenal Tilaran Conservation Area</rdfs:label>
    </owl:NamedIndividual>
    


    <!-- http://purl.obolibrary.org/obo/GAZ_00068892 -->

    <owl:NamedIndividual rdf:about="http://purl.obolibrary.org/obo/GAZ_00068892">
        <obo:RO_0001025 rdf:resource="http://purl.obolibrary.org/obo/GAZ_00003205"/>
        <obo:RO_0001025 rdf:resource="http://purl.obolibrary.org/obo/GAZ_00068891"/>
        <obo:IAO_0000115>A nature reserve in the central part of Costa Rica, which forms part of the Arenal Tilaran Conservation Area, which protects tropical forest area near San Ramon. The reserve is the site of a research station that operates under the direction of the University of Costa Rica.</obo:IAO_0000115>
        <oboInOwl:hasOBONamespace>GAZ</oboInOwl:hasOBONamespace>
        <oboInOwl:id>GAZ:00068892</oboInOwl:id>
        <rdfs:label>Alberto Manuel Brenes Biological Reserve</rdfs:label>
    </owl:NamedIndividual>
    


    <!-- http://purl.obolibrary.org/obo/GAZ_00068893 -->

    <owl:NamedIndividual rdf:about="http://purl.obolibrary.org/obo/GAZ_00068893">
        <obo:RO_0001025 rdf:resource="http://purl.obolibrary.org/obo/GAZ_00003210"/>
        <obo:RO_0001025 rdf:resource="http://purl.obolibrary.org/obo/GAZ_00068655"/>
        <obo:RO_0001025 rdf:resource="http://purl.obolibrary.org/obo/GAZ_00068891"/>
        <obo:IAO_0000115>A wildlife refuge in the central part of Costa Rica, which forms part of the Arenal Tilaran Conservation Area and protects humid forest in the Cordillera de Tilaran near Juntas.</obo:IAO_0000115>
        <oboInOwl:hasOBONamespace>GAZ</oboInOwl:hasOBONamespace>
        <oboInOwl:id>GAZ:00068893</oboInOwl:id>
        <rdfs:label>Curi Cancha Wildlife Refuge</rdfs:label>
    </owl:NamedIndividual>
    


    <!-- http://purl.obolibrary.org/obo/GAZ_00068895 -->

    <owl:NamedIndividual rdf:about="http://purl.obolibrary.org/obo/GAZ_00068895">
        <obo:RO_0001025 rdf:resource="http://purl.obolibrary.org/obo/GAZ_00068891"/>
        <obo:IAO_0000115>A nature reserve in the central part of Costa Rica, which forms part of the Arenal Tilaran Conservation Area. The site contains the Miravalles Volcano, which is still active although the last recorded eruption was only of steam vents in 1946.</obo:IAO_0000115>
        <oboInOwl:hasOBONamespace>GAZ</oboInOwl:hasOBONamespace>
        <oboInOwl:id>GAZ:00068895</oboInOwl:id>
        <rdfs:label>Miravalles Protected Zone</rdfs:label>
    </owl:NamedIndividual>
    


    <!-- http://purl.obolibrary.org/obo/GAZ_00068896 -->

    <owl:NamedIndividual rdf:about="http://purl.obolibrary.org/obo/GAZ_00068896">
        <obo:RO_0001025 rdf:resource="http://purl.obolibrary.org/obo/GAZ_00056221"/>
        <obo:RO_0001025 rdf:resource="http://purl.obolibrary.org/obo/GAZ_00068891"/>
        <obo:IAO_0000115>A national park in the central part of Costa Rica, forming the Arenal Tilaran Conservation Area. The park encompasses the Arenal Volcano the most active in the country, which had previously been believed to be dormant until a major eruption in 1968. It neighbours Lake Arenal which is the site of the country&apos;s largest hydroelectricity project, the Lake Arenal Dam.</obo:IAO_0000115>
        <oboInOwl:hasOBONamespace>GAZ</oboInOwl:hasOBONamespace>
        <oboInOwl:id>GAZ:00068896</oboInOwl:id>
        <rdfs:label>Parque Nacional Volcan Arenal</rdfs:label>
    </owl:NamedIndividual>
    


    <!-- http://purl.obolibrary.org/obo/GAZ_00068897 -->

    <owl:NamedIndividual rdf:about="http://purl.obolibrary.org/obo/GAZ_00068897">
        <obo:RO_0001025 rdf:resource="http://purl.obolibrary.org/obo/GAZ_00002901"/>
        <obo:IAO_0000115>An administrative area which is managed by the Sistema Nacional de Areas de Conservacion for the purposes of conservation in the central part of Costa Rica, notably the volcanic areas of the Cordillera Central. It contains four National Parks, and a number Wildlife refuges and other types of nature reserve.</obo:IAO_0000115>
        <oboInOwl:hasOBONamespace>GAZ</oboInOwl:hasOBONamespace>
        <oboInOwl:id>GAZ:00068897</oboInOwl:id>
        <rdfs:label>Central Volcanic Conservation Area</rdfs:label>
    </owl:NamedIndividual>
    


    <!-- http://purl.obolibrary.org/obo/GAZ_00068898 -->

    <owl:NamedIndividual rdf:about="http://purl.obolibrary.org/obo/GAZ_00068898">
        <obo:RO_0001025 rdf:resource="http://purl.obolibrary.org/obo/GAZ_00003211"/>
        <obo:RO_0001025 rdf:resource="http://purl.obolibrary.org/obo/GAZ_00068897"/>
        <obo:IAO_0000115>A protected area that includes the La Selva Biological Station. A nature reserve that protects about 15 km2 of primary tropical rainforest.</obo:IAO_0000115>
        <oboInOwl:hasOBONamespace>GAZ</oboInOwl:hasOBONamespace>
        <oboInOwl:id>GAZ:00068898</oboInOwl:id>
        <rdfs:label>La Marta Wildlife Refuge</rdfs:label>
    </owl:NamedIndividual>
    


    <!-- http://purl.obolibrary.org/obo/GAZ_00068899 -->

    <owl:NamedIndividual rdf:about="http://purl.obolibrary.org/obo/GAZ_00068899">
        <obo:RO_0001025 rdf:resource="http://purl.obolibrary.org/obo/GAZ_00003211"/>
        <obo:RO_0001025 rdf:resource="http://purl.obolibrary.org/obo/GAZ_00068897"/>
        <obo:IAO_0000115>An area that protects an ecological bridge between the Central Valley and the Talamanca Mountain Range of Costa Rica.</obo:IAO_0000115>
        <oboInOwl:hasOBONamespace>GAZ</oboInOwl:hasOBONamespace>
        <oboInOwl:id>GAZ:00068899</oboInOwl:id>
        <rdfs:label>Cerros de la Carpintera Protected Zone</rdfs:label>
    </owl:NamedIndividual>
    


    <!-- http://purl.obolibrary.org/obo/GAZ_00068900 -->

    <owl:NamedIndividual rdf:about="http://purl.obolibrary.org/obo/GAZ_00068900">
        <obo:RO_0001025 rdf:resource="http://purl.obolibrary.org/obo/GAZ_00003208"/>
        <obo:RO_0001025 rdf:resource="http://purl.obolibrary.org/obo/GAZ_00068897"/>
        <obo:IAO_0000115>A protected area located just south of Barva Volcano.</obo:IAO_0000115>
        <oboInOwl:hasOBONamespace>GAZ</oboInOwl:hasOBONamespace>
        <oboInOwl:id>GAZ:00068900</oboInOwl:id>
        <rdfs:label>Jaguarundi Wildlife Refuge</rdfs:label>
    </owl:NamedIndividual>
    


    <!-- http://purl.obolibrary.org/obo/GAZ_00068901 -->

    <owl:NamedIndividual rdf:about="http://purl.obolibrary.org/obo/GAZ_00068901">
        <obo:RO_0001025 rdf:resource="http://purl.obolibrary.org/obo/GAZ_00003205"/>
        <obo:RO_0001025 rdf:resource="http://purl.obolibrary.org/obo/GAZ_00068897"/>
        <obo:IAO_0000115>A protected area.</obo:IAO_0000115>
        <oboInOwl:hasOBONamespace>GAZ</oboInOwl:hasOBONamespace>
        <oboInOwl:id>GAZ:00068901</oboInOwl:id>
        <rdfs:label>Grecia Forest Reserve</rdfs:label>
    </owl:NamedIndividual>
    


    <!-- http://purl.obolibrary.org/obo/GAZ_00068902 -->

    <owl:NamedIndividual rdf:about="http://purl.obolibrary.org/obo/GAZ_00068902">
        <obo:RO_0001025 rdf:resource="http://purl.obolibrary.org/obo/GAZ_00003205"/>
        <obo:RO_0001025 rdf:resource="http://purl.obolibrary.org/obo/GAZ_00068897"/>
        <obo:IAO_0000115>A protected area.</obo:IAO_0000115>
        <oboInOwl:hasOBONamespace>GAZ</oboInOwl:hasOBONamespace>
        <oboInOwl:id>GAZ:00068902</oboInOwl:id>
        <rdfs:label>Cerro Atenas Protected Zone</rdfs:label>
    </owl:NamedIndividual>
    


    <!-- http://purl.obolibrary.org/obo/GAZ_00068903 -->

    <owl:NamedIndividual rdf:about="http://purl.obolibrary.org/obo/GAZ_00068903">
        <obo:RO_0001025 rdf:resource="http://purl.obolibrary.org/obo/GAZ_00068897"/>
        <oboInOwl:hasOBONamespace>GAZ</oboInOwl:hasOBONamespace>
        <oboInOwl:id>GAZ:00068903</oboInOwl:id>
        <rdfs:label>Central Volcanic Forest Reserve</rdfs:label>
    </owl:NamedIndividual>
    


    <!-- http://purl.obolibrary.org/obo/GAZ_00068904 -->

    <owl:NamedIndividual rdf:about="http://purl.obolibrary.org/obo/GAZ_00068904">
        <obo:RO_0001025 rdf:resource="http://purl.obolibrary.org/obo/GAZ_00003208"/>
        <obo:RO_0001025 rdf:resource="http://purl.obolibrary.org/obo/GAZ_00068897"/>
        <obo:IAO_0000115>A protected area in the foothills of Cerro Chompipe, southeast of Barva Volcano.</obo:IAO_0000115>
        <oboInOwl:hasOBONamespace>GAZ</oboInOwl:hasOBONamespace>
        <oboInOwl:id>GAZ:00068904</oboInOwl:id>
        <rdfs:label>Cerro Dantas Wildlife Refuge</rdfs:label>
    </owl:NamedIndividual>
    


    <!-- http://purl.obolibrary.org/obo/GAZ_00068905 -->

    <owl:NamedIndividual rdf:about="http://purl.obolibrary.org/obo/GAZ_00068905">
        <obo:RO_0001025 rdf:resource="http://purl.obolibrary.org/obo/GAZ_00003205"/>
        <obo:RO_0001025 rdf:resource="http://purl.obolibrary.org/obo/GAZ_00068897"/>
        <oboInOwl:hasOBONamespace>GAZ</oboInOwl:hasOBONamespace>
        <oboInOwl:id>GAZ:00068905</oboInOwl:id>
        <rdfs:label>Bosque Alegre Wildlife Refuge</rdfs:label>
    </owl:NamedIndividual>
    


    <!-- http://purl.obolibrary.org/obo/GAZ_00068906 -->

    <owl:NamedIndividual rdf:about="http://purl.obolibrary.org/obo/GAZ_00068906">
        <obo:RO_0001025 rdf:resource="http://purl.obolibrary.org/obo/GAZ_00009455"/>
        <obo:RO_0001025 rdf:resource="http://purl.obolibrary.org/obo/GAZ_00068897"/>
        <obo:IAO_0000115>A national park in the Central Volcanic Conservation Area of Costa Rica that encompasses the area around the Turrialba Volcano in Cartago Province.</obo:IAO_0000115>
        <oboInOwl:hasOBONamespace>GAZ</oboInOwl:hasOBONamespace>
        <oboInOwl:id>GAZ:00068906</oboInOwl:id>
        <rdfs:label>Parque Nacional Volcan Turrialba</rdfs:label>
    </owl:NamedIndividual>
    


    <!-- http://purl.obolibrary.org/obo/GAZ_00068907 -->

    <owl:NamedIndividual rdf:about="http://purl.obolibrary.org/obo/GAZ_00068907">
        <obo:RO_0001025 rdf:resource="http://purl.obolibrary.org/obo/GAZ_00068910"/>
        <obo:IAO_0000115>A protected area.</obo:IAO_0000115>
        <oboInOwl:hasOBONamespace>GAZ</oboInOwl:hasOBONamespace>
        <oboInOwl:id>GAZ:00068907</oboInOwl:id>
        <rdfs:label>Prusia Forest Reserve</rdfs:label>
    </owl:NamedIndividual>
    


    <!-- http://purl.obolibrary.org/obo/GAZ_00068908 -->

    <owl:NamedIndividual rdf:about="http://purl.obolibrary.org/obo/GAZ_00068908">
        <obo:RO_0001025 rdf:resource="http://purl.obolibrary.org/obo/GAZ_00003208"/>
        <obo:RO_0001025 rdf:resource="http://purl.obolibrary.org/obo/GAZ_00068897"/>
        <obo:IAO_0000115>A protected area of lowland tropical rainforest bordering Braulio Carrillo National Park, between the Sarapiqui and Puerto Viejo Rivers. The Organization for Tropical Studies administers a Biological Station in this protected zone.</obo:IAO_0000115>
        <oboInOwl:hasOBONamespace>GAZ</oboInOwl:hasOBONamespace>
        <oboInOwl:id>GAZ:00068908</oboInOwl:id>
        <rdfs:label>La Selva Protected Zone</rdfs:label>
    </owl:NamedIndividual>
    


    <!-- http://purl.obolibrary.org/obo/GAZ_00068909 -->

    <owl:NamedIndividual rdf:about="http://purl.obolibrary.org/obo/GAZ_00068909">
        <obo:RO_0001025 rdf:resource="http://purl.obolibrary.org/obo/GAZ_00003211"/>
        <obo:RO_0001025 rdf:resource="http://purl.obolibrary.org/obo/GAZ_00068897"/>
        <obo:IAO_0000115>An archeological site. A national monument in the Central Volcanic Conservation Area in the Cartago Province of Costa Rica that covers the largest archaeological site in the country.</obo:IAO_0000115>
        <oboInOwl:hasOBONamespace>GAZ</oboInOwl:hasOBONamespace>
        <oboInOwl:id>GAZ:00068909</oboInOwl:id>
        <rdfs:label>Guayabo National Monument</rdfs:label>
    </owl:NamedIndividual>
    


    <!-- http://purl.obolibrary.org/obo/GAZ_00068910 -->

    <owl:NamedIndividual rdf:about="http://purl.obolibrary.org/obo/GAZ_00068910">
        <obo:RO_0001025 rdf:resource="http://purl.obolibrary.org/obo/GAZ_00003211"/>
        <obo:RO_0001025 rdf:resource="http://purl.obolibrary.org/obo/GAZ_00068897"/>
        <obo:IAO_0000115>A national park in the Central Volcanic Conservation Area of Costa Rica that encompasses the area around the Irazu Volcano in Cartago Province which incorporates what used to be the Ruben Torres Rojas Forest Reserve now called the Prusia Forest Reserve.</obo:IAO_0000115>
        <oboInOwl:hasOBONamespace>GAZ</oboInOwl:hasOBONamespace>
        <oboInOwl:id>GAZ:00068910</oboInOwl:id>
        <rdfs:label>Parque Nacional Volcan Irazu</rdfs:label>
    </owl:NamedIndividual>
    


    <!-- http://purl.obolibrary.org/obo/GAZ_00068911 -->

    <owl:NamedIndividual rdf:about="http://purl.obolibrary.org/obo/GAZ_00068911">
        <obo:RO_0001025 rdf:resource="http://purl.obolibrary.org/obo/GAZ_00003210"/>
        <obo:RO_0001025 rdf:resource="http://purl.obolibrary.org/obo/GAZ_00068682"/>
        <obo:IAO_0000115>A national park in the western part of Costa Rica, which forms part of the Tempisque Conservation Area about 12 km from the Tempisque River. It was created in 1974.</obo:IAO_0000115>
        <oboInOwl:hasOBONamespace>GAZ</oboInOwl:hasOBONamespace>
        <oboInOwl:id>GAZ:00068911</oboInOwl:id>
        <rdfs:label>Barra Honda National Park</rdfs:label>
    </owl:NamedIndividual>
    


    <!-- http://purl.obolibrary.org/obo/GAZ_00090259 -->

    <owl:NamedIndividual rdf:about="http://purl.obolibrary.org/obo/GAZ_00090259">
        <obo:IAO_0000115>A national park.</obo:IAO_0000115>
        <oboInOwl:hasOBONamespace>GAZ</oboInOwl:hasOBONamespace>
        <oboInOwl:id>GAZ:00090259</oboInOwl:id>
        <rdfs:label>Parque Nacional Volcan Baru</rdfs:label>
    </owl:NamedIndividual>
    


    <!-- http://purl.obolibrary.org/obo/GAZ_00118866 -->

    <owl:NamedIndividual rdf:about="http://purl.obolibrary.org/obo/GAZ_00118866">
        <rdf:type rdf:resource="http://purl.obolibrary.org/obo/ENVO_00000004"/>
        <obo:RO_0001025 rdf:resource="http://purl.obolibrary.org/obo/GAZ_00068658"/>
        <obo:IAO_0000115>A district of Alajuela Canton.</obo:IAO_0000115>
        <oboInOwl:hasOBONamespace>GAZ</oboInOwl:hasOBONamespace>
        <oboInOwl:id>GAZ:00118866</oboInOwl:id>
        <rdfs:label>Alajuela District</rdfs:label>
    </owl:NamedIndividual>
    


    <!-- http://purl.obolibrary.org/obo/GAZ_00118867 -->

    <owl:NamedIndividual rdf:about="http://purl.obolibrary.org/obo/GAZ_00118867">
        <rdf:type rdf:resource="http://purl.obolibrary.org/obo/ENVO_00000004"/>
        <obo:RO_0001025 rdf:resource="http://purl.obolibrary.org/obo/GAZ_00068658"/>
        <obo:IAO_0000115>A district of Alajuela Canton.</obo:IAO_0000115>
        <oboInOwl:hasOBONamespace>GAZ</oboInOwl:hasOBONamespace>
        <oboInOwl:id>GAZ:00118867</oboInOwl:id>
        <rdfs:label>Tambor District</rdfs:label>
    </owl:NamedIndividual>
    


    <!-- http://purl.obolibrary.org/obo/GAZ_00118868 -->

    <owl:NamedIndividual rdf:about="http://purl.obolibrary.org/obo/GAZ_00118868">
        <rdf:type rdf:resource="http://purl.obolibrary.org/obo/ENVO_00000004"/>
        <obo:RO_0001025 rdf:resource="http://purl.obolibrary.org/obo/GAZ_00068658"/>
        <obo:IAO_0000115>A district of Alajuela Canton.</obo:IAO_0000115>
        <oboInOwl:hasOBONamespace>GAZ</oboInOwl:hasOBONamespace>
        <oboInOwl:id>GAZ:00118868</oboInOwl:id>
        <rdfs:label>Sarapiqui District</rdfs:label>
    </owl:NamedIndividual>
    


    <!-- http://purl.obolibrary.org/obo/GAZ_00118869 -->

    <owl:NamedIndividual rdf:about="http://purl.obolibrary.org/obo/GAZ_00118869">
        <rdf:type rdf:resource="http://purl.obolibrary.org/obo/ENVO_00000004"/>
        <obo:RO_0001025 rdf:resource="http://purl.obolibrary.org/obo/GAZ_00068658"/>
        <obo:IAO_0000115>A district of Alajuela Canton.</obo:IAO_0000115>
        <oboInOwl:hasOBONamespace>GAZ</oboInOwl:hasOBONamespace>
        <oboInOwl:id>GAZ:00118869</oboInOwl:id>
        <rdfs:label>Rio Segundo District</rdfs:label>
    </owl:NamedIndividual>
    


    <!-- http://purl.obolibrary.org/obo/GAZ_00118870 -->

    <owl:NamedIndividual rdf:about="http://purl.obolibrary.org/obo/GAZ_00118870">
        <rdf:type rdf:resource="http://purl.obolibrary.org/obo/ENVO_00000004"/>
        <obo:RO_0001025 rdf:resource="http://purl.obolibrary.org/obo/GAZ_00068658"/>
        <obo:IAO_0000115>A district of Alajuela Canton.</obo:IAO_0000115>
        <oboInOwl:hasOBONamespace>GAZ</oboInOwl:hasOBONamespace>
        <oboInOwl:id>GAZ:00118870</oboInOwl:id>
        <rdfs:label>Desamparados District</rdfs:label>
    </owl:NamedIndividual>
    


    <!-- http://purl.obolibrary.org/obo/GAZ_00118871 -->

    <owl:NamedIndividual rdf:about="http://purl.obolibrary.org/obo/GAZ_00118871">
        <rdf:type rdf:resource="http://purl.obolibrary.org/obo/ENVO_00000004"/>
        <obo:RO_0001025 rdf:resource="http://purl.obolibrary.org/obo/GAZ_00068658"/>
        <obo:IAO_0000115>A district of Alajuela Canton.</obo:IAO_0000115>
        <oboInOwl:hasOBONamespace>GAZ</oboInOwl:hasOBONamespace>
        <oboInOwl:id>GAZ:00118871</oboInOwl:id>
        <rdfs:label>San Rafael District</rdfs:label>
    </owl:NamedIndividual>
    


    <!-- http://purl.obolibrary.org/obo/GAZ_00118872 -->

    <owl:NamedIndividual rdf:about="http://purl.obolibrary.org/obo/GAZ_00118872">
        <rdf:type rdf:resource="http://purl.obolibrary.org/obo/ENVO_00000004"/>
        <obo:RO_0001025 rdf:resource="http://purl.obolibrary.org/obo/GAZ_00068658"/>
        <obo:IAO_0000115>A district of Alajuela Canton.</obo:IAO_0000115>
        <oboInOwl:hasOBONamespace>GAZ</oboInOwl:hasOBONamespace>
        <oboInOwl:id>GAZ:00118872</oboInOwl:id>
        <rdfs:label>La Garita District</rdfs:label>
    </owl:NamedIndividual>
    


    <!-- http://purl.obolibrary.org/obo/GAZ_00118873 -->

    <owl:NamedIndividual rdf:about="http://purl.obolibrary.org/obo/GAZ_00118873">
        <rdf:type rdf:resource="http://purl.obolibrary.org/obo/ENVO_00000004"/>
        <obo:RO_0001025 rdf:resource="http://purl.obolibrary.org/obo/GAZ_00068658"/>
        <obo:IAO_0000115>A district of Alajuela Canton.</obo:IAO_0000115>
        <oboInOwl:hasOBONamespace>GAZ</oboInOwl:hasOBONamespace>
        <oboInOwl:id>GAZ:00118873</oboInOwl:id>
        <rdfs:label>Sabanilla District</rdfs:label>
    </owl:NamedIndividual>
    


    <!-- http://purl.obolibrary.org/obo/GAZ_00118874 -->

    <owl:NamedIndividual rdf:about="http://purl.obolibrary.org/obo/GAZ_00118874">
        <rdf:type rdf:resource="http://purl.obolibrary.org/obo/ENVO_00000004"/>
        <obo:RO_0001025 rdf:resource="http://purl.obolibrary.org/obo/GAZ_00068658"/>
        <obo:IAO_0000115>A district of Alajuela Canton.</obo:IAO_0000115>
        <oboInOwl:hasOBONamespace>GAZ</oboInOwl:hasOBONamespace>
        <oboInOwl:id>GAZ:00118874</oboInOwl:id>
        <rdfs:label>Turrucares District</rdfs:label>
    </owl:NamedIndividual>
    


    <!-- http://purl.obolibrary.org/obo/GAZ_00118875 -->

    <owl:NamedIndividual rdf:about="http://purl.obolibrary.org/obo/GAZ_00118875">
        <rdf:type rdf:resource="http://purl.obolibrary.org/obo/ENVO_00000004"/>
        <obo:RO_0001025 rdf:resource="http://purl.obolibrary.org/obo/GAZ_00068658"/>
        <obo:IAO_0000115>A district of Alajuela Canton.</obo:IAO_0000115>
        <oboInOwl:hasOBONamespace>GAZ</oboInOwl:hasOBONamespace>
        <oboInOwl:id>GAZ:00118875</oboInOwl:id>
        <rdfs:label>La Guacima District</rdfs:label>
    </owl:NamedIndividual>
    


    <!-- http://purl.obolibrary.org/obo/GAZ_00118876 -->

    <owl:NamedIndividual rdf:about="http://purl.obolibrary.org/obo/GAZ_00118876">
        <rdf:type rdf:resource="http://purl.obolibrary.org/obo/ENVO_00000004"/>
        <obo:RO_0001025 rdf:resource="http://purl.obolibrary.org/obo/GAZ_00068658"/>
        <obo:IAO_0000115>A district of Alajuela Canton.</obo:IAO_0000115>
        <oboInOwl:hasOBONamespace>GAZ</oboInOwl:hasOBONamespace>
        <oboInOwl:id>GAZ:00118876</oboInOwl:id>
        <rdfs:label>San Jose District</rdfs:label>
    </owl:NamedIndividual>
    


    <!-- http://purl.obolibrary.org/obo/GAZ_00118877 -->

    <owl:NamedIndividual rdf:about="http://purl.obolibrary.org/obo/GAZ_00118877">
        <rdf:type rdf:resource="http://purl.obolibrary.org/obo/ENVO_00000004"/>
        <obo:RO_0001025 rdf:resource="http://purl.obolibrary.org/obo/GAZ_00068658"/>
        <obo:IAO_0000115>A district of Alajuela Canton.</obo:IAO_0000115>
        <oboInOwl:hasOBONamespace>GAZ</oboInOwl:hasOBONamespace>
        <oboInOwl:id>GAZ:00118877</oboInOwl:id>
        <rdfs:label>Carrizal District</rdfs:label>
    </owl:NamedIndividual>
    


    <!-- http://purl.obolibrary.org/obo/GAZ_00118878 -->

    <owl:NamedIndividual rdf:about="http://purl.obolibrary.org/obo/GAZ_00118878">
        <rdf:type rdf:resource="http://purl.obolibrary.org/obo/ENVO_00000004"/>
        <obo:RO_0001025 rdf:resource="http://purl.obolibrary.org/obo/GAZ_00068658"/>
        <obo:IAO_0000115>A district of Alajuela Canton.</obo:IAO_0000115>
        <oboInOwl:hasOBONamespace>GAZ</oboInOwl:hasOBONamespace>
        <oboInOwl:id>GAZ:00118878</oboInOwl:id>
        <rdfs:label>San Antonio de Tejar District</rdfs:label>
    </owl:NamedIndividual>
    


    <!-- http://purl.obolibrary.org/obo/GAZ_00118879 -->

    <owl:NamedIndividual rdf:about="http://purl.obolibrary.org/obo/GAZ_00118879">
        <rdf:type rdf:resource="http://purl.obolibrary.org/obo/ENVO_00000004"/>
        <obo:RO_0001025 rdf:resource="http://purl.obolibrary.org/obo/GAZ_00068658"/>
        <obo:IAO_0000115>A district of Alajuela Canton.</obo:IAO_0000115>
        <oboInOwl:hasOBONamespace>GAZ</oboInOwl:hasOBONamespace>
        <oboInOwl:id>GAZ:00118879</oboInOwl:id>
        <rdfs:label>San Isidro District</rdfs:label>
    </owl:NamedIndividual>
    


    <!-- http://purl.obolibrary.org/obo/GAZ_00118880 -->

    <owl:NamedIndividual rdf:about="http://purl.obolibrary.org/obo/GAZ_00118880">
        <rdf:type rdf:resource="http://purl.obolibrary.org/obo/ENVO_00000004"/>
        <obo:RO_0001025 rdf:resource="http://purl.obolibrary.org/obo/GAZ_00056221"/>
        <obo:IAO_0000115>A district of San Carlos Canton.</obo:IAO_0000115>
        <oboInOwl:hasOBONamespace>GAZ</oboInOwl:hasOBONamespace>
        <oboInOwl:id>GAZ:00118880</oboInOwl:id>
        <rdfs:label>Quesada District</rdfs:label>
    </owl:NamedIndividual>
    


    <!-- http://purl.obolibrary.org/obo/GAZ_00118881 -->

    <owl:NamedIndividual rdf:about="http://purl.obolibrary.org/obo/GAZ_00118881">
        <rdf:type rdf:resource="http://purl.obolibrary.org/obo/ENVO_00000004"/>
        <obo:RO_0001025 rdf:resource="http://purl.obolibrary.org/obo/GAZ_00056221"/>
        <obo:IAO_0000115>A district of San Carlos Canton.</obo:IAO_0000115>
        <oboInOwl:hasOBONamespace>GAZ</oboInOwl:hasOBONamespace>
        <oboInOwl:id>GAZ:00118881</oboInOwl:id>
        <rdfs:label>Pocosol District</rdfs:label>
    </owl:NamedIndividual>
    


    <!-- http://purl.obolibrary.org/obo/GAZ_00118882 -->

    <owl:NamedIndividual rdf:about="http://purl.obolibrary.org/obo/GAZ_00118882">
        <rdf:type rdf:resource="http://purl.obolibrary.org/obo/ENVO_00000004"/>
        <obo:RO_0001025 rdf:resource="http://purl.obolibrary.org/obo/GAZ_00056221"/>
        <obo:IAO_0000115>A district of San Carlos Canton.</obo:IAO_0000115>
        <oboInOwl:hasOBONamespace>GAZ</oboInOwl:hasOBONamespace>
        <oboInOwl:id>GAZ:00118882</oboInOwl:id>
        <rdfs:label>La Palmera District</rdfs:label>
    </owl:NamedIndividual>
    


    <!-- http://purl.obolibrary.org/obo/GAZ_00118883 -->

    <owl:NamedIndividual rdf:about="http://purl.obolibrary.org/obo/GAZ_00118883">
        <rdf:type rdf:resource="http://purl.obolibrary.org/obo/ENVO_00000004"/>
        <obo:RO_0001025 rdf:resource="http://purl.obolibrary.org/obo/GAZ_00056221"/>
        <obo:IAO_0000115>A district of San Carlos Canton.</obo:IAO_0000115>
        <oboInOwl:hasOBONamespace>GAZ</oboInOwl:hasOBONamespace>
        <oboInOwl:id>GAZ:00118883</oboInOwl:id>
        <rdfs:label>Venado District</rdfs:label>
    </owl:NamedIndividual>
    


    <!-- http://purl.obolibrary.org/obo/GAZ_00118884 -->

    <owl:NamedIndividual rdf:about="http://purl.obolibrary.org/obo/GAZ_00118884">
        <rdf:type rdf:resource="http://purl.obolibrary.org/obo/ENVO_00000004"/>
        <obo:RO_0001025 rdf:resource="http://purl.obolibrary.org/obo/GAZ_00056221"/>
        <obo:IAO_0000115>A district of San Carlos Canton.</obo:IAO_0000115>
        <oboInOwl:hasOBONamespace>GAZ</oboInOwl:hasOBONamespace>
        <oboInOwl:id>GAZ:00118884</oboInOwl:id>
        <rdfs:label>Venecia District</rdfs:label>
    </owl:NamedIndividual>
    


    <!-- http://purl.obolibrary.org/obo/GAZ_00118885 -->

    <owl:NamedIndividual rdf:about="http://purl.obolibrary.org/obo/GAZ_00118885">
        <rdf:type rdf:resource="http://purl.obolibrary.org/obo/ENVO_00000004"/>
        <obo:RO_0001025 rdf:resource="http://purl.obolibrary.org/obo/GAZ_00056221"/>
        <obo:IAO_0000115>A district of San Carlos Canton.</obo:IAO_0000115>
        <oboInOwl:hasOBONamespace>GAZ</oboInOwl:hasOBONamespace>
        <oboInOwl:id>GAZ:00118885</oboInOwl:id>
        <rdfs:label>Monterrey District</rdfs:label>
    </owl:NamedIndividual>
    


    <!-- http://purl.obolibrary.org/obo/GAZ_00118886 -->

    <owl:NamedIndividual rdf:about="http://purl.obolibrary.org/obo/GAZ_00118886">
        <rdf:type rdf:resource="http://purl.obolibrary.org/obo/ENVO_00000004"/>
        <obo:RO_0001025 rdf:resource="http://purl.obolibrary.org/obo/GAZ_00056221"/>
        <obo:IAO_0000115>A district of San Carlos Canton.</obo:IAO_0000115>
        <oboInOwl:hasOBONamespace>GAZ</oboInOwl:hasOBONamespace>
        <oboInOwl:id>GAZ:00118886</oboInOwl:id>
        <rdfs:label>Florencia District</rdfs:label>
    </owl:NamedIndividual>
    


    <!-- http://purl.obolibrary.org/obo/GAZ_00118887 -->

    <owl:NamedIndividual rdf:about="http://purl.obolibrary.org/obo/GAZ_00118887">
        <rdf:type rdf:resource="http://purl.obolibrary.org/obo/ENVO_00000004"/>
        <obo:RO_0001025 rdf:resource="http://purl.obolibrary.org/obo/GAZ_00056221"/>
        <obo:IAO_0000115>A district of San Carlos Canton.</obo:IAO_0000115>
        <oboInOwl:hasOBONamespace>GAZ</oboInOwl:hasOBONamespace>
        <oboInOwl:id>GAZ:00118887</oboInOwl:id>
        <rdfs:label>Pital District</rdfs:label>
    </owl:NamedIndividual>
    


    <!-- http://purl.obolibrary.org/obo/GAZ_00118888 -->

    <owl:NamedIndividual rdf:about="http://purl.obolibrary.org/obo/GAZ_00118888">
        <rdf:type rdf:resource="http://purl.obolibrary.org/obo/ENVO_00000004"/>
        <obo:RO_0001025 rdf:resource="http://purl.obolibrary.org/obo/GAZ_00056221"/>
        <obo:IAO_0000115>A district of San Carlos Canton.</obo:IAO_0000115>
        <oboInOwl:hasOBONamespace>GAZ</oboInOwl:hasOBONamespace>
        <oboInOwl:id>GAZ:00118888</oboInOwl:id>
        <rdfs:label>La Tigra District</rdfs:label>
    </owl:NamedIndividual>
    


    <!-- http://purl.obolibrary.org/obo/GAZ_00118889 -->

    <owl:NamedIndividual rdf:about="http://purl.obolibrary.org/obo/GAZ_00118889">
        <rdf:type rdf:resource="http://purl.obolibrary.org/obo/ENVO_00000004"/>
        <obo:RO_0001025 rdf:resource="http://purl.obolibrary.org/obo/GAZ_00056221"/>
        <obo:IAO_0000115>A district of San Carlos Canton.</obo:IAO_0000115>
        <oboInOwl:hasOBONamespace>GAZ</oboInOwl:hasOBONamespace>
        <oboInOwl:id>GAZ:00118889</oboInOwl:id>
        <rdfs:label>Cutris District</rdfs:label>
    </owl:NamedIndividual>
    


    <!-- http://purl.obolibrary.org/obo/GAZ_00118890 -->

    <owl:NamedIndividual rdf:about="http://purl.obolibrary.org/obo/GAZ_00118890">
        <rdf:type rdf:resource="http://purl.obolibrary.org/obo/ENVO_00000004"/>
        <obo:RO_0001025 rdf:resource="http://purl.obolibrary.org/obo/GAZ_00056221"/>
        <obo:IAO_0000115>A district of San Carlos Canton.</obo:IAO_0000115>
        <oboInOwl:hasOBONamespace>GAZ</oboInOwl:hasOBONamespace>
        <oboInOwl:id>GAZ:00118890</oboInOwl:id>
        <rdfs:label>La Fortuna District</rdfs:label>
    </owl:NamedIndividual>
    


    <!-- http://purl.obolibrary.org/obo/GAZ_00118891 -->

    <owl:NamedIndividual rdf:about="http://purl.obolibrary.org/obo/GAZ_00118891">
        <rdf:type rdf:resource="http://purl.obolibrary.org/obo/ENVO_00000004"/>
        <obo:RO_0001025 rdf:resource="http://purl.obolibrary.org/obo/GAZ_00056221"/>
        <obo:IAO_0000115>A district of San Carlos Canton.</obo:IAO_0000115>
        <oboInOwl:hasOBONamespace>GAZ</oboInOwl:hasOBONamespace>
        <oboInOwl:id>GAZ:00118891</oboInOwl:id>
        <rdfs:label>Buenavista District</rdfs:label>
    </owl:NamedIndividual>
    


    <!-- http://purl.obolibrary.org/obo/GAZ_00118892 -->

    <owl:NamedIndividual rdf:about="http://purl.obolibrary.org/obo/GAZ_00118892">
        <rdf:type rdf:resource="http://purl.obolibrary.org/obo/ENVO_00000004"/>
        <obo:RO_0001025 rdf:resource="http://purl.obolibrary.org/obo/GAZ_00056221"/>
        <obo:IAO_0000115>A district of San Carlos Canton.</obo:IAO_0000115>
        <oboInOwl:hasOBONamespace>GAZ</oboInOwl:hasOBONamespace>
        <oboInOwl:id>GAZ:00118892</oboInOwl:id>
        <rdfs:label>Aguas Zarcas District</rdfs:label>
    </owl:NamedIndividual>
    


    <!-- http://purl.obolibrary.org/obo/GAZ_00118893 -->

    <owl:NamedIndividual rdf:about="http://purl.obolibrary.org/obo/GAZ_00118893">
        <rdf:type rdf:resource="http://purl.obolibrary.org/obo/ENVO_00000004"/>
        <obo:RO_0001025 rdf:resource="http://purl.obolibrary.org/obo/GAZ_00068652"/>
        <obo:IAO_0000115>A district of San Ramon Canton.</obo:IAO_0000115>
        <oboInOwl:hasOBONamespace>GAZ</oboInOwl:hasOBONamespace>
        <oboInOwl:id>GAZ:00118893</oboInOwl:id>
        <rdfs:label>San Ramon District</rdfs:label>
    </owl:NamedIndividual>
    


    <!-- http://purl.obolibrary.org/obo/GAZ_00118894 -->

    <owl:NamedIndividual rdf:about="http://purl.obolibrary.org/obo/GAZ_00118894">
        <rdf:type rdf:resource="http://purl.obolibrary.org/obo/ENVO_00000004"/>
        <obo:RO_0001025 rdf:resource="http://purl.obolibrary.org/obo/GAZ_00068652"/>
        <obo:IAO_0000115>A district of San Ramon Canton.</obo:IAO_0000115>
        <oboInOwl:hasOBONamespace>GAZ</oboInOwl:hasOBONamespace>
        <oboInOwl:id>GAZ:00118894</oboInOwl:id>
        <rdfs:label>Concepcion District</rdfs:label>
    </owl:NamedIndividual>
    


    <!-- http://purl.obolibrary.org/obo/GAZ_00118895 -->

    <owl:NamedIndividual rdf:about="http://purl.obolibrary.org/obo/GAZ_00118895">
        <rdf:type rdf:resource="http://purl.obolibrary.org/obo/ENVO_00000004"/>
        <obo:RO_0001025 rdf:resource="http://purl.obolibrary.org/obo/GAZ_00068652"/>
        <obo:IAO_0000115>A district of San Ramon Canton.</obo:IAO_0000115>
        <oboInOwl:hasOBONamespace>GAZ</oboInOwl:hasOBONamespace>
        <oboInOwl:id>GAZ:00118895</oboInOwl:id>
        <rdfs:label>Penas Blancas District</rdfs:label>
    </owl:NamedIndividual>
    


    <!-- http://purl.obolibrary.org/obo/GAZ_00118896 -->

    <owl:NamedIndividual rdf:about="http://purl.obolibrary.org/obo/GAZ_00118896">
        <rdf:type rdf:resource="http://purl.obolibrary.org/obo/ENVO_00000004"/>
        <obo:RO_0001025 rdf:resource="http://purl.obolibrary.org/obo/GAZ_00068652"/>
        <obo:IAO_0000115>A district of San Ramon Canton.</obo:IAO_0000115>
        <oboInOwl:hasOBONamespace>GAZ</oboInOwl:hasOBONamespace>
        <oboInOwl:id>GAZ:00118896</oboInOwl:id>
        <rdfs:label>Alfaro District</rdfs:label>
    </owl:NamedIndividual>
    


    <!-- http://purl.obolibrary.org/obo/GAZ_00118897 -->

    <owl:NamedIndividual rdf:about="http://purl.obolibrary.org/obo/GAZ_00118897">
        <rdf:type rdf:resource="http://purl.obolibrary.org/obo/ENVO_00000004"/>
        <obo:RO_0001025 rdf:resource="http://purl.obolibrary.org/obo/GAZ_00068652"/>
        <obo:IAO_0000115>A district of San Ramon Canton.</obo:IAO_0000115>
        <oboInOwl:hasOBONamespace>GAZ</oboInOwl:hasOBONamespace>
        <oboInOwl:id>GAZ:00118897</oboInOwl:id>
        <rdfs:label>Zapotal District</rdfs:label>
    </owl:NamedIndividual>
    


    <!-- http://purl.obolibrary.org/obo/GAZ_00118898 -->

    <owl:NamedIndividual rdf:about="http://purl.obolibrary.org/obo/GAZ_00118898">
        <rdf:type rdf:resource="http://purl.obolibrary.org/obo/ENVO_00000004"/>
        <obo:RO_0001025 rdf:resource="http://purl.obolibrary.org/obo/GAZ_00068652"/>
        <obo:IAO_0000115>A district of San Ramon Canton.</obo:IAO_0000115>
        <oboInOwl:hasOBONamespace>GAZ</oboInOwl:hasOBONamespace>
        <oboInOwl:id>GAZ:00118898</oboInOwl:id>
        <rdfs:label>San Rafael District</rdfs:label>
    </owl:NamedIndividual>
    


    <!-- http://purl.obolibrary.org/obo/GAZ_00118899 -->

    <owl:NamedIndividual rdf:about="http://purl.obolibrary.org/obo/GAZ_00118899">
        <rdf:type rdf:resource="http://purl.obolibrary.org/obo/ENVO_00000004"/>
        <obo:RO_0001025 rdf:resource="http://purl.obolibrary.org/obo/GAZ_00068652"/>
        <obo:IAO_0000115>A district of San Ramon Canton.</obo:IAO_0000115>
        <oboInOwl:hasOBONamespace>GAZ</oboInOwl:hasOBONamespace>
        <oboInOwl:id>GAZ:00118899</oboInOwl:id>
        <rdfs:label>Volio District</rdfs:label>
    </owl:NamedIndividual>
    


    <!-- http://purl.obolibrary.org/obo/GAZ_00118900 -->

    <owl:NamedIndividual rdf:about="http://purl.obolibrary.org/obo/GAZ_00118900">
        <rdf:type rdf:resource="http://purl.obolibrary.org/obo/ENVO_00000004"/>
        <obo:RO_0001025 rdf:resource="http://purl.obolibrary.org/obo/GAZ_00068652"/>
        <obo:IAO_0000115>A district of San Ramon Canton.</obo:IAO_0000115>
        <oboInOwl:hasOBONamespace>GAZ</oboInOwl:hasOBONamespace>
        <oboInOwl:id>GAZ:00118900</oboInOwl:id>
        <rdfs:label>Los Angeles District</rdfs:label>
    </owl:NamedIndividual>
    


    <!-- http://purl.obolibrary.org/obo/GAZ_00118901 -->

    <owl:NamedIndividual rdf:about="http://purl.obolibrary.org/obo/GAZ_00118901">
        <rdf:type rdf:resource="http://purl.obolibrary.org/obo/ENVO_00000004"/>
        <obo:RO_0001025 rdf:resource="http://purl.obolibrary.org/obo/GAZ_00068652"/>
        <obo:IAO_0000115>A district of San Ramon Canton.</obo:IAO_0000115>
        <oboInOwl:hasOBONamespace>GAZ</oboInOwl:hasOBONamespace>
        <oboInOwl:id>GAZ:00118901</oboInOwl:id>
        <rdfs:label>Piedades Norte District</rdfs:label>
    </owl:NamedIndividual>
    


    <!-- http://purl.obolibrary.org/obo/GAZ_00118902 -->

    <owl:NamedIndividual rdf:about="http://purl.obolibrary.org/obo/GAZ_00118902">
        <rdf:type rdf:resource="http://purl.obolibrary.org/obo/ENVO_00000004"/>
        <obo:RO_0001025 rdf:resource="http://purl.obolibrary.org/obo/GAZ_00068652"/>
        <obo:IAO_0000115>A district of San Ramon Canton.</obo:IAO_0000115>
        <oboInOwl:hasOBONamespace>GAZ</oboInOwl:hasOBONamespace>
        <oboInOwl:id>GAZ:00118902</oboInOwl:id>
        <rdfs:label>San Isidro District</rdfs:label>
    </owl:NamedIndividual>
    


    <!-- http://purl.obolibrary.org/obo/GAZ_00118903 -->

    <owl:NamedIndividual rdf:about="http://purl.obolibrary.org/obo/GAZ_00118903">
        <rdf:type rdf:resource="http://purl.obolibrary.org/obo/ENVO_00000004"/>
        <obo:RO_0001025 rdf:resource="http://purl.obolibrary.org/obo/GAZ_00068652"/>
        <obo:IAO_0000115>A district of San Ramon Canton.</obo:IAO_0000115>
        <oboInOwl:hasOBONamespace>GAZ</oboInOwl:hasOBONamespace>
        <oboInOwl:id>GAZ:00118903</oboInOwl:id>
        <rdfs:label>Santiago District</rdfs:label>
    </owl:NamedIndividual>
    


    <!-- http://purl.obolibrary.org/obo/GAZ_00118904 -->

    <owl:NamedIndividual rdf:about="http://purl.obolibrary.org/obo/GAZ_00118904">
        <rdf:type rdf:resource="http://purl.obolibrary.org/obo/ENVO_00000004"/>
        <obo:RO_0001025 rdf:resource="http://purl.obolibrary.org/obo/GAZ_00068652"/>
        <obo:IAO_0000115>A district of San Ramon Canton.</obo:IAO_0000115>
        <oboInOwl:hasOBONamespace>GAZ</oboInOwl:hasOBONamespace>
        <oboInOwl:id>GAZ:00118904</oboInOwl:id>
        <rdfs:label>San Juan District</rdfs:label>
    </owl:NamedIndividual>
    


    <!-- http://purl.obolibrary.org/obo/GAZ_00118905 -->

    <owl:NamedIndividual rdf:about="http://purl.obolibrary.org/obo/GAZ_00118905">
        <rdf:type rdf:resource="http://purl.obolibrary.org/obo/ENVO_00000004"/>
        <obo:RO_0001025 rdf:resource="http://purl.obolibrary.org/obo/GAZ_00068650"/>
        <obo:IAO_0000115>A district of San Mateo Canton.</obo:IAO_0000115>
        <oboInOwl:hasOBONamespace>GAZ</oboInOwl:hasOBONamespace>
        <oboInOwl:id>GAZ:00118905</oboInOwl:id>
        <rdfs:label>Desmonte District</rdfs:label>
    </owl:NamedIndividual>
    


    <!-- http://purl.obolibrary.org/obo/GAZ_00118906 -->

    <owl:NamedIndividual rdf:about="http://purl.obolibrary.org/obo/GAZ_00118906">
        <rdf:type rdf:resource="http://purl.obolibrary.org/obo/ENVO_00000004"/>
        <obo:RO_0001025 rdf:resource="http://purl.obolibrary.org/obo/GAZ_00068652"/>
        <obo:IAO_0000115>A district of San Ramon Canton.</obo:IAO_0000115>
        <oboInOwl:hasOBONamespace>GAZ</oboInOwl:hasOBONamespace>
        <oboInOwl:id>GAZ:00118906</oboInOwl:id>
        <rdfs:label>Piedades Sur District</rdfs:label>
    </owl:NamedIndividual>
    


    <!-- http://purl.obolibrary.org/obo/GAZ_00118907 -->

    <owl:NamedIndividual rdf:about="http://purl.obolibrary.org/obo/GAZ_00118907">
        <rdf:type rdf:resource="http://purl.obolibrary.org/obo/ENVO_00000004"/>
        <obo:RO_0001025 rdf:resource="http://purl.obolibrary.org/obo/GAZ_00068648"/>
        <obo:IAO_0000115>A district of Grecia Canton.</obo:IAO_0000115>
        <oboInOwl:hasOBONamespace>GAZ</oboInOwl:hasOBONamespace>
        <oboInOwl:id>GAZ:00118907</oboInOwl:id>
        <rdfs:label>Rio Cuarto District</rdfs:label>
    </owl:NamedIndividual>
    


    <!-- http://purl.obolibrary.org/obo/GAZ_00118908 -->

    <owl:NamedIndividual rdf:about="http://purl.obolibrary.org/obo/GAZ_00118908">
        <rdf:type rdf:resource="http://purl.obolibrary.org/obo/ENVO_00000004"/>
        <obo:RO_0001025 rdf:resource="http://purl.obolibrary.org/obo/GAZ_00068648"/>
        <obo:IAO_0000115>A district of Grecia Canton.</obo:IAO_0000115>
        <oboInOwl:hasOBONamespace>GAZ</oboInOwl:hasOBONamespace>
        <oboInOwl:id>GAZ:00118908</oboInOwl:id>
        <rdfs:label>San Jose District</rdfs:label>
    </owl:NamedIndividual>
    


    <!-- http://purl.obolibrary.org/obo/GAZ_00118909 -->

    <owl:NamedIndividual rdf:about="http://purl.obolibrary.org/obo/GAZ_00118909">
        <rdf:type rdf:resource="http://purl.obolibrary.org/obo/ENVO_00000004"/>
        <obo:RO_0001025 rdf:resource="http://purl.obolibrary.org/obo/GAZ_00068648"/>
        <obo:IAO_0000115>A district of Grecia Canton.</obo:IAO_0000115>
        <oboInOwl:hasOBONamespace>GAZ</oboInOwl:hasOBONamespace>
        <oboInOwl:id>GAZ:00118909</oboInOwl:id>
        <rdfs:label>Grecia District</rdfs:label>
    </owl:NamedIndividual>
    


    <!-- http://purl.obolibrary.org/obo/GAZ_00118910 -->

    <owl:NamedIndividual rdf:about="http://purl.obolibrary.org/obo/GAZ_00118910">
        <rdf:type rdf:resource="http://purl.obolibrary.org/obo/ENVO_00000004"/>
        <obo:RO_0001025 rdf:resource="http://purl.obolibrary.org/obo/GAZ_00068648"/>
        <obo:IAO_0000115>A district of Grecia Canton.</obo:IAO_0000115>
        <oboInOwl:hasOBONamespace>GAZ</oboInOwl:hasOBONamespace>
        <oboInOwl:id>GAZ:00118910</oboInOwl:id>
        <rdfs:label>San Isidro District</rdfs:label>
    </owl:NamedIndividual>
    


    <!-- http://purl.obolibrary.org/obo/GAZ_00118911 -->

    <owl:NamedIndividual rdf:about="http://purl.obolibrary.org/obo/GAZ_00118911">
        <rdf:type rdf:resource="http://purl.obolibrary.org/obo/ENVO_00000004"/>
        <obo:RO_0001025 rdf:resource="http://purl.obolibrary.org/obo/GAZ_00068648"/>
        <obo:IAO_0000115>A district of Grecia Canton.</obo:IAO_0000115>
        <oboInOwl:hasOBONamespace>GAZ</oboInOwl:hasOBONamespace>
        <oboInOwl:id>GAZ:00118911</oboInOwl:id>
        <rdfs:label>Bolivar District</rdfs:label>
    </owl:NamedIndividual>
    


    <!-- http://purl.obolibrary.org/obo/GAZ_00118912 -->

    <owl:NamedIndividual rdf:about="http://purl.obolibrary.org/obo/GAZ_00118912">
        <rdf:type rdf:resource="http://purl.obolibrary.org/obo/ENVO_00000004"/>
        <obo:RO_0001025 rdf:resource="http://purl.obolibrary.org/obo/GAZ_00068648"/>
        <obo:IAO_0000115>A district of Grecia Canton.</obo:IAO_0000115>
        <oboInOwl:hasOBONamespace>GAZ</oboInOwl:hasOBONamespace>
        <oboInOwl:id>GAZ:00118912</oboInOwl:id>
        <rdfs:label>Puente de Piedra District</rdfs:label>
    </owl:NamedIndividual>
    


    <!-- http://purl.obolibrary.org/obo/GAZ_00118913 -->

    <owl:NamedIndividual rdf:about="http://purl.obolibrary.org/obo/GAZ_00118913">
        <rdf:type rdf:resource="http://purl.obolibrary.org/obo/ENVO_00000004"/>
        <obo:RO_0001025 rdf:resource="http://purl.obolibrary.org/obo/GAZ_00068648"/>
        <obo:IAO_0000115>A district of Grecia Canton.</obo:IAO_0000115>
        <oboInOwl:hasOBONamespace>GAZ</oboInOwl:hasOBONamespace>
        <oboInOwl:id>GAZ:00118913</oboInOwl:id>
        <rdfs:label>Tacares District</rdfs:label>
    </owl:NamedIndividual>
    


    <!-- http://purl.obolibrary.org/obo/GAZ_00118914 -->

    <owl:NamedIndividual rdf:about="http://purl.obolibrary.org/obo/GAZ_00118914">
        <rdf:type rdf:resource="http://purl.obolibrary.org/obo/ENVO_00000004"/>
        <obo:RO_0001025 rdf:resource="http://purl.obolibrary.org/obo/GAZ_00068648"/>
        <obo:IAO_0000115>A district of Grecia Canton.</obo:IAO_0000115>
        <oboInOwl:hasOBONamespace>GAZ</oboInOwl:hasOBONamespace>
        <oboInOwl:id>GAZ:00118914</oboInOwl:id>
        <rdfs:label>San Roque District</rdfs:label>
    </owl:NamedIndividual>
    


    <!-- http://purl.obolibrary.org/obo/GAZ_00118915 -->

    <owl:NamedIndividual rdf:about="http://purl.obolibrary.org/obo/GAZ_00118915">
        <rdf:type rdf:resource="http://purl.obolibrary.org/obo/ENVO_00000004"/>
        <obo:RO_0001025 rdf:resource="http://purl.obolibrary.org/obo/GAZ_00068656"/>
        <obo:IAO_0000115>A district of Upala Canton.</obo:IAO_0000115>
        <oboInOwl:hasOBONamespace>GAZ</oboInOwl:hasOBONamespace>
        <oboInOwl:id>GAZ:00118915</oboInOwl:id>
        <rdfs:label>Upala District</rdfs:label>
    </owl:NamedIndividual>
    


    <!-- http://purl.obolibrary.org/obo/GAZ_00118916 -->

    <owl:NamedIndividual rdf:about="http://purl.obolibrary.org/obo/GAZ_00118916">
        <rdf:type rdf:resource="http://purl.obolibrary.org/obo/ENVO_00000004"/>
        <obo:RO_0001025 rdf:resource="http://purl.obolibrary.org/obo/GAZ_00068656"/>
        <obo:IAO_0000115>A district of Upala Canton.</obo:IAO_0000115>
        <oboInOwl:hasOBONamespace>GAZ</oboInOwl:hasOBONamespace>
        <oboInOwl:id>GAZ:00118916</oboInOwl:id>
        <rdfs:label>Bijagua District</rdfs:label>
    </owl:NamedIndividual>
    


    <!-- http://purl.obolibrary.org/obo/GAZ_00118917 -->

    <owl:NamedIndividual rdf:about="http://purl.obolibrary.org/obo/GAZ_00118917">
        <rdf:type rdf:resource="http://purl.obolibrary.org/obo/ENVO_00000004"/>
        <obo:RO_0001025 rdf:resource="http://purl.obolibrary.org/obo/GAZ_00068656"/>
        <obo:IAO_0000115>A district of Upala Canton.</obo:IAO_0000115>
        <oboInOwl:hasOBONamespace>GAZ</oboInOwl:hasOBONamespace>
        <oboInOwl:id>GAZ:00118917</oboInOwl:id>
        <rdfs:label>Yolillal District</rdfs:label>
    </owl:NamedIndividual>
    


    <!-- http://purl.obolibrary.org/obo/GAZ_00118918 -->

    <owl:NamedIndividual rdf:about="http://purl.obolibrary.org/obo/GAZ_00118918">
        <rdf:type rdf:resource="http://purl.obolibrary.org/obo/ENVO_00000004"/>
        <obo:RO_0001025 rdf:resource="http://purl.obolibrary.org/obo/GAZ_00068656"/>
        <obo:IAO_0000115>A district of Upala Canton.</obo:IAO_0000115>
        <oboInOwl:hasOBONamespace>GAZ</oboInOwl:hasOBONamespace>
        <oboInOwl:id>GAZ:00118918</oboInOwl:id>
        <rdfs:label>San Jose District</rdfs:label>
    </owl:NamedIndividual>
    


    <!-- http://purl.obolibrary.org/obo/GAZ_00118919 -->

    <owl:NamedIndividual rdf:about="http://purl.obolibrary.org/obo/GAZ_00118919">
        <rdf:type rdf:resource="http://purl.obolibrary.org/obo/ENVO_00000004"/>
        <obo:RO_0001025 rdf:resource="http://purl.obolibrary.org/obo/GAZ_00068656"/>
        <obo:IAO_0000115>A district of Upala Canton.</obo:IAO_0000115>
        <oboInOwl:hasOBONamespace>GAZ</oboInOwl:hasOBONamespace>
        <oboInOwl:id>GAZ:00118919</oboInOwl:id>
        <rdfs:label>Dos Rios District</rdfs:label>
    </owl:NamedIndividual>
    


    <!-- http://purl.obolibrary.org/obo/GAZ_00118920 -->

    <owl:NamedIndividual rdf:about="http://purl.obolibrary.org/obo/GAZ_00118920">
        <rdf:type rdf:resource="http://purl.obolibrary.org/obo/ENVO_00000004"/>
        <obo:RO_0001025 rdf:resource="http://purl.obolibrary.org/obo/GAZ_00068656"/>
        <obo:IAO_0000115>A district of Upala Canton.</obo:IAO_0000115>
        <oboInOwl:hasOBONamespace>GAZ</oboInOwl:hasOBONamespace>
        <oboInOwl:id>GAZ:00118920</oboInOwl:id>
        <rdfs:label>Aguas Claras District</rdfs:label>
    </owl:NamedIndividual>
    


    <!-- http://purl.obolibrary.org/obo/GAZ_00118921 -->

    <owl:NamedIndividual rdf:about="http://purl.obolibrary.org/obo/GAZ_00118921">
        <rdf:type rdf:resource="http://purl.obolibrary.org/obo/ENVO_00000004"/>
        <obo:RO_0001025 rdf:resource="http://purl.obolibrary.org/obo/GAZ_00068656"/>
        <obo:IAO_0000115>A district of Upala Canton.</obo:IAO_0000115>
        <oboInOwl:hasOBONamespace>GAZ</oboInOwl:hasOBONamespace>
        <oboInOwl:id>GAZ:00118921</oboInOwl:id>
        <rdfs:label>Delicias District</rdfs:label>
    </owl:NamedIndividual>
    


    <!-- http://purl.obolibrary.org/obo/GAZ_00118922 -->

    <owl:NamedIndividual rdf:about="http://purl.obolibrary.org/obo/GAZ_00118922">
        <rdf:type rdf:resource="http://purl.obolibrary.org/obo/ENVO_00000004"/>
        <obo:RO_0001025 rdf:resource="http://purl.obolibrary.org/obo/GAZ_00068646"/>
        <obo:IAO_0000115>A district of Naranjo Canton.</obo:IAO_0000115>
        <oboInOwl:hasOBONamespace>GAZ</oboInOwl:hasOBONamespace>
        <oboInOwl:id>GAZ:00118922</oboInOwl:id>
        <rdfs:label>Naranjo de Alajuela District</rdfs:label>
    </owl:NamedIndividual>
    


    <!-- http://purl.obolibrary.org/obo/GAZ_00118923 -->

    <owl:NamedIndividual rdf:about="http://purl.obolibrary.org/obo/GAZ_00118923">
        <rdf:type rdf:resource="http://purl.obolibrary.org/obo/ENVO_00000004"/>
        <obo:RO_0001025 rdf:resource="http://purl.obolibrary.org/obo/GAZ_00068646"/>
        <obo:IAO_0000115>A district of Naranjo Canton.</obo:IAO_0000115>
        <oboInOwl:hasOBONamespace>GAZ</oboInOwl:hasOBONamespace>
        <oboInOwl:id>GAZ:00118923</oboInOwl:id>
        <rdfs:label>San Miguel District</rdfs:label>
    </owl:NamedIndividual>
    


    <!-- http://purl.obolibrary.org/obo/GAZ_00118924 -->

    <owl:NamedIndividual rdf:about="http://purl.obolibrary.org/obo/GAZ_00118924">
        <rdf:type rdf:resource="http://purl.obolibrary.org/obo/ENVO_00000004"/>
        <obo:RO_0001025 rdf:resource="http://purl.obolibrary.org/obo/GAZ_00068646"/>
        <obo:IAO_0000115>A district of Naranjo Canton.</obo:IAO_0000115>
        <oboInOwl:hasOBONamespace>GAZ</oboInOwl:hasOBONamespace>
        <oboInOwl:id>GAZ:00118924</oboInOwl:id>
        <rdfs:label>El Rosario District</rdfs:label>
    </owl:NamedIndividual>
    


    <!-- http://purl.obolibrary.org/obo/GAZ_00118925 -->

    <owl:NamedIndividual rdf:about="http://purl.obolibrary.org/obo/GAZ_00118925">
        <rdf:type rdf:resource="http://purl.obolibrary.org/obo/ENVO_00000004"/>
        <obo:RO_0001025 rdf:resource="http://purl.obolibrary.org/obo/GAZ_00068646"/>
        <obo:IAO_0000115>A district of Naranjo Canton.</obo:IAO_0000115>
        <oboInOwl:hasOBONamespace>GAZ</oboInOwl:hasOBONamespace>
        <oboInOwl:id>GAZ:00118925</oboInOwl:id>
        <rdfs:label>San Juan District</rdfs:label>
    </owl:NamedIndividual>
    


    <!-- http://purl.obolibrary.org/obo/GAZ_00118926 -->

    <owl:NamedIndividual rdf:about="http://purl.obolibrary.org/obo/GAZ_00118926">
        <rdf:type rdf:resource="http://purl.obolibrary.org/obo/ENVO_00000004"/>
        <obo:RO_0001025 rdf:resource="http://purl.obolibrary.org/obo/GAZ_00068646"/>
        <obo:IAO_0000115>A district of Naranjo Canton.</obo:IAO_0000115>
        <oboInOwl:hasOBONamespace>GAZ</oboInOwl:hasOBONamespace>
        <oboInOwl:id>GAZ:00118926</oboInOwl:id>
        <rdfs:label>Cirri Sur District</rdfs:label>
    </owl:NamedIndividual>
    


    <!-- http://purl.obolibrary.org/obo/GAZ_00118927 -->

    <owl:NamedIndividual rdf:about="http://purl.obolibrary.org/obo/GAZ_00118927">
        <rdf:type rdf:resource="http://purl.obolibrary.org/obo/ENVO_00000004"/>
        <obo:RO_0001025 rdf:resource="http://purl.obolibrary.org/obo/GAZ_00068646"/>
        <obo:IAO_0000115>A district of Naranjo Canton.</obo:IAO_0000115>
        <oboInOwl:hasOBONamespace>GAZ</oboInOwl:hasOBONamespace>
        <oboInOwl:id>GAZ:00118927</oboInOwl:id>
        <rdfs:label>San Jeronimo District</rdfs:label>
    </owl:NamedIndividual>
    


    <!-- http://purl.obolibrary.org/obo/GAZ_00118928 -->

    <owl:NamedIndividual rdf:about="http://purl.obolibrary.org/obo/GAZ_00118928">
        <rdf:type rdf:resource="http://purl.obolibrary.org/obo/ENVO_00000004"/>
        <obo:RO_0001025 rdf:resource="http://purl.obolibrary.org/obo/GAZ_00068646"/>
        <obo:IAO_0000115>A district of Naranjo Canton.</obo:IAO_0000115>
        <oboInOwl:hasOBONamespace>GAZ</oboInOwl:hasOBONamespace>
        <oboInOwl:id>GAZ:00118928</oboInOwl:id>
        <rdfs:label>San Jose District</rdfs:label>
    </owl:NamedIndividual>
    


    <!-- http://purl.obolibrary.org/obo/GAZ_00118929 -->

    <owl:NamedIndividual rdf:about="http://purl.obolibrary.org/obo/GAZ_00118929">
        <rdf:type rdf:resource="http://purl.obolibrary.org/obo/ENVO_00000004"/>
        <obo:RO_0001025 rdf:resource="http://purl.obolibrary.org/obo/GAZ_00068650"/>
        <obo:IAO_0000115>A district of San Mateo Canton.</obo:IAO_0000115>
        <oboInOwl:hasOBONamespace>GAZ</oboInOwl:hasOBONamespace>
        <oboInOwl:id>GAZ:00118929</oboInOwl:id>
        <rdfs:label>San Mateo District</rdfs:label>
    </owl:NamedIndividual>
    


    <!-- http://purl.obolibrary.org/obo/GAZ_00118930 -->

    <owl:NamedIndividual rdf:about="http://purl.obolibrary.org/obo/GAZ_00118930">
        <rdf:type rdf:resource="http://purl.obolibrary.org/obo/ENVO_00000004"/>
        <obo:RO_0001025 rdf:resource="http://purl.obolibrary.org/obo/GAZ_00068650"/>
        <obo:IAO_0000115>A district of San Mateo Canton.</obo:IAO_0000115>
        <oboInOwl:hasOBONamespace>GAZ</oboInOwl:hasOBONamespace>
        <oboInOwl:id>GAZ:00118930</oboInOwl:id>
        <rdfs:label>Jesus Maria District</rdfs:label>
    </owl:NamedIndividual>
    


    <!-- http://purl.obolibrary.org/obo/GAZ_00118931 -->

    <owl:NamedIndividual rdf:about="http://purl.obolibrary.org/obo/GAZ_00118931">
        <rdf:type rdf:resource="http://purl.obolibrary.org/obo/ENVO_00000004"/>
        <obo:RO_0001025 rdf:resource="http://purl.obolibrary.org/obo/GAZ_00068654"/>
        <obo:IAO_0000115>A district of Atenas Canton.</obo:IAO_0000115>
        <oboInOwl:hasOBONamespace>GAZ</oboInOwl:hasOBONamespace>
        <oboInOwl:id>GAZ:00118931</oboInOwl:id>
        <rdfs:label>Jesus District</rdfs:label>
    </owl:NamedIndividual>
    


    <!-- http://purl.obolibrary.org/obo/GAZ_00118932 -->

    <owl:NamedIndividual rdf:about="http://purl.obolibrary.org/obo/GAZ_00118932">
        <rdf:type rdf:resource="http://purl.obolibrary.org/obo/ENVO_00000004"/>
        <obo:RO_0001025 rdf:resource="http://purl.obolibrary.org/obo/GAZ_00068654"/>
        <obo:IAO_0000115>A district of Atenas Canton.</obo:IAO_0000115>
        <oboInOwl:hasOBONamespace>GAZ</oboInOwl:hasOBONamespace>
        <oboInOwl:id>GAZ:00118932</oboInOwl:id>
        <rdfs:label>San Isidro District</rdfs:label>
    </owl:NamedIndividual>
    


    <!-- http://purl.obolibrary.org/obo/GAZ_00118933 -->

    <owl:NamedIndividual rdf:about="http://purl.obolibrary.org/obo/GAZ_00118933">
        <rdf:type rdf:resource="http://purl.obolibrary.org/obo/ENVO_00000004"/>
        <obo:RO_0001025 rdf:resource="http://purl.obolibrary.org/obo/GAZ_00068654"/>
        <obo:IAO_0000115>A district of Atenas Canton.</obo:IAO_0000115>
        <oboInOwl:hasOBONamespace>GAZ</oboInOwl:hasOBONamespace>
        <oboInOwl:id>GAZ:00118933</oboInOwl:id>
        <rdfs:label>San Jose District</rdfs:label>
    </owl:NamedIndividual>
    


    <!-- http://purl.obolibrary.org/obo/GAZ_00118934 -->

    <owl:NamedIndividual rdf:about="http://purl.obolibrary.org/obo/GAZ_00118934">
        <rdf:type rdf:resource="http://purl.obolibrary.org/obo/ENVO_00000004"/>
        <obo:RO_0001025 rdf:resource="http://purl.obolibrary.org/obo/GAZ_00068654"/>
        <obo:IAO_0000115>A district of Atenas Canton.</obo:IAO_0000115>
        <oboInOwl:hasOBONamespace>GAZ</oboInOwl:hasOBONamespace>
        <oboInOwl:id>GAZ:00118934</oboInOwl:id>
        <rdfs:label>Mercedes District</rdfs:label>
    </owl:NamedIndividual>
    


    <!-- http://purl.obolibrary.org/obo/GAZ_00118935 -->

    <owl:NamedIndividual rdf:about="http://purl.obolibrary.org/obo/GAZ_00118935">
        <rdf:type rdf:resource="http://purl.obolibrary.org/obo/ENVO_00000004"/>
        <obo:RO_0001025 rdf:resource="http://purl.obolibrary.org/obo/GAZ_00068654"/>
        <obo:IAO_0000115>A district of Atenas Canton.</obo:IAO_0000115>
        <oboInOwl:hasOBONamespace>GAZ</oboInOwl:hasOBONamespace>
        <oboInOwl:id>GAZ:00118935</oboInOwl:id>
        <rdfs:label>Atenas District</rdfs:label>
    </owl:NamedIndividual>
    


    <!-- http://purl.obolibrary.org/obo/GAZ_00118936 -->

    <owl:NamedIndividual rdf:about="http://purl.obolibrary.org/obo/GAZ_00118936">
        <rdf:type rdf:resource="http://purl.obolibrary.org/obo/ENVO_00000004"/>
        <obo:RO_0001025 rdf:resource="http://purl.obolibrary.org/obo/GAZ_00068654"/>
        <obo:IAO_0000115>A district of Atenas Canton.</obo:IAO_0000115>
        <oboInOwl:hasOBONamespace>GAZ</oboInOwl:hasOBONamespace>
        <oboInOwl:id>GAZ:00118936</oboInOwl:id>
        <rdfs:label>Santa Eulalia District</rdfs:label>
    </owl:NamedIndividual>
    


    <!-- http://purl.obolibrary.org/obo/GAZ_00118937 -->

    <owl:NamedIndividual rdf:about="http://purl.obolibrary.org/obo/GAZ_00118937">
        <rdf:type rdf:resource="http://purl.obolibrary.org/obo/ENVO_00000004"/>
        <obo:RO_0001025 rdf:resource="http://purl.obolibrary.org/obo/GAZ_00068654"/>
        <obo:IAO_0000115>A district of Atenas Canton.</obo:IAO_0000115>
        <oboInOwl:hasOBONamespace>GAZ</oboInOwl:hasOBONamespace>
        <oboInOwl:id>GAZ:00118937</oboInOwl:id>
        <rdfs:label>Concepcion District</rdfs:label>
    </owl:NamedIndividual>
    


    <!-- http://purl.obolibrary.org/obo/GAZ_00118938 -->

    <owl:NamedIndividual rdf:about="http://purl.obolibrary.org/obo/GAZ_00118938">
        <rdf:type rdf:resource="http://purl.obolibrary.org/obo/ENVO_00000004"/>
        <obo:RO_0001025 rdf:resource="http://purl.obolibrary.org/obo/GAZ_00068651"/>
        <obo:IAO_0000115>A district of Palmares Canton.</obo:IAO_0000115>
        <oboInOwl:hasOBONamespace>GAZ</oboInOwl:hasOBONamespace>
        <oboInOwl:id>GAZ:00118938</oboInOwl:id>
        <rdfs:label>Santiago District</rdfs:label>
    </owl:NamedIndividual>
    


    <!-- http://purl.obolibrary.org/obo/GAZ_00118939 -->

    <owl:NamedIndividual rdf:about="http://purl.obolibrary.org/obo/GAZ_00118939">
        <rdf:type rdf:resource="http://purl.obolibrary.org/obo/ENVO_00000004"/>
        <obo:RO_0001025 rdf:resource="http://purl.obolibrary.org/obo/GAZ_00068651"/>
        <obo:IAO_0000115>A district of Palmares Canton.</obo:IAO_0000115>
        <oboInOwl:hasOBONamespace>GAZ</oboInOwl:hasOBONamespace>
        <oboInOwl:id>GAZ:00118939</oboInOwl:id>
        <rdfs:label>Granja District</rdfs:label>
    </owl:NamedIndividual>
    


    <!-- http://purl.obolibrary.org/obo/GAZ_00118940 -->

    <owl:NamedIndividual rdf:about="http://purl.obolibrary.org/obo/GAZ_00118940">
        <rdf:type rdf:resource="http://purl.obolibrary.org/obo/ENVO_00000004"/>
        <obo:RO_0001025 rdf:resource="http://purl.obolibrary.org/obo/GAZ_00068651"/>
        <obo:IAO_0000115>A district of Palmares Canton.</obo:IAO_0000115>
        <oboInOwl:hasOBONamespace>GAZ</oboInOwl:hasOBONamespace>
        <oboInOwl:id>GAZ:00118940</oboInOwl:id>
        <rdfs:label>Esquipulas District</rdfs:label>
    </owl:NamedIndividual>
    


    <!-- http://purl.obolibrary.org/obo/GAZ_00118941 -->

    <owl:NamedIndividual rdf:about="http://purl.obolibrary.org/obo/GAZ_00118941">
        <rdf:type rdf:resource="http://purl.obolibrary.org/obo/ENVO_00000004"/>
        <obo:RO_0001025 rdf:resource="http://purl.obolibrary.org/obo/GAZ_00068651"/>
        <obo:IAO_0000115>A district of Palmares Canton.</obo:IAO_0000115>
        <oboInOwl:hasOBONamespace>GAZ</oboInOwl:hasOBONamespace>
        <oboInOwl:id>GAZ:00118941</oboInOwl:id>
        <rdfs:label>Palmares Centro District</rdfs:label>
    </owl:NamedIndividual>
    


    <!-- http://purl.obolibrary.org/obo/GAZ_00118942 -->

    <owl:NamedIndividual rdf:about="http://purl.obolibrary.org/obo/GAZ_00118942">
        <rdf:type rdf:resource="http://purl.obolibrary.org/obo/ENVO_00000004"/>
        <obo:RO_0001025 rdf:resource="http://purl.obolibrary.org/obo/GAZ_00068651"/>
        <obo:IAO_0000115>A district of Palmares Canton.</obo:IAO_0000115>
        <oboInOwl:hasOBONamespace>GAZ</oboInOwl:hasOBONamespace>
        <oboInOwl:id>GAZ:00118942</oboInOwl:id>
        <rdfs:label>Zaragoza District</rdfs:label>
    </owl:NamedIndividual>
    


    <!-- http://purl.obolibrary.org/obo/GAZ_00118943 -->

    <owl:NamedIndividual rdf:about="http://purl.obolibrary.org/obo/GAZ_00118943">
        <rdf:type rdf:resource="http://purl.obolibrary.org/obo/ENVO_00000004"/>
        <obo:RO_0001025 rdf:resource="http://purl.obolibrary.org/obo/GAZ_00068651"/>
        <obo:IAO_0000115>A district of Palmares Canton.</obo:IAO_0000115>
        <oboInOwl:hasOBONamespace>GAZ</oboInOwl:hasOBONamespace>
        <oboInOwl:id>GAZ:00118943</oboInOwl:id>
        <rdfs:label>Candelaria District</rdfs:label>
    </owl:NamedIndividual>
    


    <!-- http://purl.obolibrary.org/obo/GAZ_00118944 -->

    <owl:NamedIndividual rdf:about="http://purl.obolibrary.org/obo/GAZ_00118944">
        <rdf:type rdf:resource="http://purl.obolibrary.org/obo/ENVO_00000004"/>
        <obo:RO_0001025 rdf:resource="http://purl.obolibrary.org/obo/GAZ_00068651"/>
        <obo:IAO_0000115>A district of Palmares Canton.</obo:IAO_0000115>
        <oboInOwl:hasOBONamespace>GAZ</oboInOwl:hasOBONamespace>
        <oboInOwl:id>GAZ:00118944</oboInOwl:id>
        <rdfs:label>Buenos Aires District</rdfs:label>
    </owl:NamedIndividual>
    


    <!-- http://purl.obolibrary.org/obo/GAZ_00118945 -->

    <owl:NamedIndividual rdf:about="http://purl.obolibrary.org/obo/GAZ_00118945">
        <rdf:type rdf:resource="http://purl.obolibrary.org/obo/ENVO_00000004"/>
        <obo:RO_0001025 rdf:resource="http://purl.obolibrary.org/obo/GAZ_00068645"/>
        <obo:IAO_0000115>A district of Poas Canton.</obo:IAO_0000115>
        <oboInOwl:hasOBONamespace>GAZ</oboInOwl:hasOBONamespace>
        <oboInOwl:id>GAZ:00118945</oboInOwl:id>
        <rdfs:label>San Juan District</rdfs:label>
    </owl:NamedIndividual>
    


    <!-- http://purl.obolibrary.org/obo/GAZ_00118946 -->

    <owl:NamedIndividual rdf:about="http://purl.obolibrary.org/obo/GAZ_00118946">
        <rdf:type rdf:resource="http://purl.obolibrary.org/obo/ENVO_00000004"/>
        <obo:RO_0001025 rdf:resource="http://purl.obolibrary.org/obo/GAZ_00068645"/>
        <obo:IAO_0000115>A district of Poas Canton.</obo:IAO_0000115>
        <oboInOwl:hasOBONamespace>GAZ</oboInOwl:hasOBONamespace>
        <oboInOwl:id>GAZ:00118946</oboInOwl:id>
        <rdfs:label>San Pedro de Poas District</rdfs:label>
    </owl:NamedIndividual>
    


    <!-- http://purl.obolibrary.org/obo/GAZ_00118947 -->

    <owl:NamedIndividual rdf:about="http://purl.obolibrary.org/obo/GAZ_00118947">
        <rdf:type rdf:resource="http://purl.obolibrary.org/obo/ENVO_00000004"/>
        <obo:RO_0001025 rdf:resource="http://purl.obolibrary.org/obo/GAZ_00068645"/>
        <obo:IAO_0000115>A district of Poas Canton.</obo:IAO_0000115>
        <oboInOwl:hasOBONamespace>GAZ</oboInOwl:hasOBONamespace>
        <oboInOwl:id>GAZ:00118947</oboInOwl:id>
        <rdfs:label>Carrillos District</rdfs:label>
    </owl:NamedIndividual>
    


    <!-- http://purl.obolibrary.org/obo/GAZ_00118948 -->

    <owl:NamedIndividual rdf:about="http://purl.obolibrary.org/obo/GAZ_00118948">
        <rdf:type rdf:resource="http://purl.obolibrary.org/obo/ENVO_00000004"/>
        <obo:RO_0001025 rdf:resource="http://purl.obolibrary.org/obo/GAZ_00068645"/>
        <obo:IAO_0000115>A district of Poas Canton.</obo:IAO_0000115>
        <oboInOwl:hasOBONamespace>GAZ</oboInOwl:hasOBONamespace>
        <oboInOwl:id>GAZ:00118948</oboInOwl:id>
        <rdfs:label>Sabana Redonda District</rdfs:label>
    </owl:NamedIndividual>
    


    <!-- http://purl.obolibrary.org/obo/GAZ_00118949 -->

    <owl:NamedIndividual rdf:about="http://purl.obolibrary.org/obo/GAZ_00118949">
        <rdf:type rdf:resource="http://purl.obolibrary.org/obo/ENVO_00000004"/>
        <obo:RO_0001025 rdf:resource="http://purl.obolibrary.org/obo/GAZ_00068645"/>
        <obo:IAO_0000115>A district of Poas Canton.</obo:IAO_0000115>
        <oboInOwl:hasOBONamespace>GAZ</oboInOwl:hasOBONamespace>
        <oboInOwl:id>GAZ:00118949</oboInOwl:id>
        <rdfs:label>San Rafael District</rdfs:label>
    </owl:NamedIndividual>
    


    <!-- http://purl.obolibrary.org/obo/GAZ_00118950 -->

    <owl:NamedIndividual rdf:about="http://purl.obolibrary.org/obo/GAZ_00118950">
        <rdf:type rdf:resource="http://purl.obolibrary.org/obo/ENVO_00000004"/>
        <obo:RO_0001025 rdf:resource="http://purl.obolibrary.org/obo/GAZ_00068657"/>
        <obo:IAO_0000115>A district of Orotina Canton.</obo:IAO_0000115>
        <oboInOwl:hasOBONamespace>GAZ</oboInOwl:hasOBONamespace>
        <oboInOwl:id>GAZ:00118950</oboInOwl:id>
        <rdfs:label>Mastatea District</rdfs:label>
    </owl:NamedIndividual>
    


    <!-- http://purl.obolibrary.org/obo/GAZ_00118951 -->

    <owl:NamedIndividual rdf:about="http://purl.obolibrary.org/obo/GAZ_00118951">
        <rdf:type rdf:resource="http://purl.obolibrary.org/obo/ENVO_00000004"/>
        <obo:RO_0001025 rdf:resource="http://purl.obolibrary.org/obo/GAZ_00068657"/>
        <obo:IAO_0000115>A district of Orotina Canton.</obo:IAO_0000115>
        <oboInOwl:hasOBONamespace>GAZ</oboInOwl:hasOBONamespace>
        <oboInOwl:id>GAZ:00118951</oboInOwl:id>
        <rdfs:label>Coyolara District</rdfs:label>
    </owl:NamedIndividual>
    


    <!-- http://purl.obolibrary.org/obo/GAZ_00118952 -->

    <owl:NamedIndividual rdf:about="http://purl.obolibrary.org/obo/GAZ_00118952">
        <rdf:type rdf:resource="http://purl.obolibrary.org/obo/ENVO_00000004"/>
        <obo:RO_0001025 rdf:resource="http://purl.obolibrary.org/obo/GAZ_00068657"/>
        <obo:IAO_0000115>A district of Orotina Canton.</obo:IAO_0000115>
        <oboInOwl:hasOBONamespace>GAZ</oboInOwl:hasOBONamespace>
        <oboInOwl:id>GAZ:00118952</oboInOwl:id>
        <rdfs:label>Orotina District</rdfs:label>
    </owl:NamedIndividual>
    


    <!-- http://purl.obolibrary.org/obo/GAZ_00118953 -->

    <owl:NamedIndividual rdf:about="http://purl.obolibrary.org/obo/GAZ_00118953">
        <rdf:type rdf:resource="http://purl.obolibrary.org/obo/ENVO_00000004"/>
        <obo:RO_0001025 rdf:resource="http://purl.obolibrary.org/obo/GAZ_00068657"/>
        <obo:IAO_0000115>A district of Orotina Canton.</obo:IAO_0000115>
        <oboInOwl:hasOBONamespace>GAZ</oboInOwl:hasOBONamespace>
        <oboInOwl:id>GAZ:00118953</oboInOwl:id>
        <rdfs:label>Ceibaa District</rdfs:label>
    </owl:NamedIndividual>
    


    <!-- http://purl.obolibrary.org/obo/GAZ_00118954 -->

    <owl:NamedIndividual rdf:about="http://purl.obolibrary.org/obo/GAZ_00118954">
        <rdf:type rdf:resource="http://purl.obolibrary.org/obo/ENVO_00000004"/>
        <obo:RO_0001025 rdf:resource="http://purl.obolibrary.org/obo/GAZ_00068657"/>
        <obo:IAO_0000115>A district of Orotina Canton.</obo:IAO_0000115>
        <oboInOwl:hasOBONamespace>GAZ</oboInOwl:hasOBONamespace>
        <oboInOwl:id>GAZ:00118954</oboInOwl:id>
        <rdfs:label>Hacienda Viejaa District</rdfs:label>
    </owl:NamedIndividual>
    


    <!-- http://purl.obolibrary.org/obo/GAZ_00118955 -->

    <owl:NamedIndividual rdf:about="http://purl.obolibrary.org/obo/GAZ_00118955">
        <rdf:type rdf:resource="http://purl.obolibrary.org/obo/ENVO_00000004"/>
        <obo:RO_0001025 rdf:resource="http://purl.obolibrary.org/obo/GAZ_00068659"/>
        <obo:IAO_0000115>A district of Alfaro Ruiz Canton.</obo:IAO_0000115>
        <oboInOwl:hasOBONamespace>GAZ</oboInOwl:hasOBONamespace>
        <oboInOwl:id>GAZ:00118955</oboInOwl:id>
        <rdfs:label>Guadalupe District</rdfs:label>
    </owl:NamedIndividual>
    


    <!-- http://purl.obolibrary.org/obo/GAZ_00118956 -->

    <owl:NamedIndividual rdf:about="http://purl.obolibrary.org/obo/GAZ_00118956">
        <rdf:type rdf:resource="http://purl.obolibrary.org/obo/ENVO_00000004"/>
        <obo:RO_0001025 rdf:resource="http://purl.obolibrary.org/obo/GAZ_00068659"/>
        <obo:IAO_0000115>A district of Alfaro Ruiz Canton.</obo:IAO_0000115>
        <oboInOwl:hasOBONamespace>GAZ</oboInOwl:hasOBONamespace>
        <oboInOwl:id>GAZ:00118956</oboInOwl:id>
        <rdfs:label>Palmira District</rdfs:label>
    </owl:NamedIndividual>
    


    <!-- http://purl.obolibrary.org/obo/GAZ_00118957 -->

    <owl:NamedIndividual rdf:about="http://purl.obolibrary.org/obo/GAZ_00118957">
        <rdf:type rdf:resource="http://purl.obolibrary.org/obo/ENVO_00000004"/>
        <obo:RO_0001025 rdf:resource="http://purl.obolibrary.org/obo/GAZ_00068659"/>
        <obo:IAO_0000115>A district of Alfaro Ruiz Canton.</obo:IAO_0000115>
        <oboInOwl:hasOBONamespace>GAZ</oboInOwl:hasOBONamespace>
        <oboInOwl:id>GAZ:00118957</oboInOwl:id>
        <rdfs:label>Laguna District</rdfs:label>
    </owl:NamedIndividual>
    


    <!-- http://purl.obolibrary.org/obo/GAZ_00118958 -->

    <owl:NamedIndividual rdf:about="http://purl.obolibrary.org/obo/GAZ_00118958">
        <rdf:type rdf:resource="http://purl.obolibrary.org/obo/ENVO_00000004"/>
        <obo:RO_0001025 rdf:resource="http://purl.obolibrary.org/obo/GAZ_00068659"/>
        <obo:IAO_0000115>A district of Alfaro Ruiz Canton.</obo:IAO_0000115>
        <oboInOwl:hasOBONamespace>GAZ</oboInOwl:hasOBONamespace>
        <oboInOwl:id>GAZ:00118958</oboInOwl:id>
        <rdfs:label>Zapote District</rdfs:label>
    </owl:NamedIndividual>
    


    <!-- http://purl.obolibrary.org/obo/GAZ_00118959 -->

    <owl:NamedIndividual rdf:about="http://purl.obolibrary.org/obo/GAZ_00118959">
        <rdf:type rdf:resource="http://purl.obolibrary.org/obo/ENVO_00000004"/>
        <obo:RO_0001025 rdf:resource="http://purl.obolibrary.org/obo/GAZ_00068659"/>
        <obo:IAO_0000115>A district of Alfaro Ruiz Canton.</obo:IAO_0000115>
        <oboInOwl:hasOBONamespace>GAZ</oboInOwl:hasOBONamespace>
        <oboInOwl:id>GAZ:00118959</oboInOwl:id>
        <rdfs:label>Zarcero District</rdfs:label>
    </owl:NamedIndividual>
    


    <!-- http://purl.obolibrary.org/obo/GAZ_00118960 -->

    <owl:NamedIndividual rdf:about="http://purl.obolibrary.org/obo/GAZ_00118960">
        <rdf:type rdf:resource="http://purl.obolibrary.org/obo/ENVO_00000004"/>
        <obo:RO_0001025 rdf:resource="http://purl.obolibrary.org/obo/GAZ_00068659"/>
        <obo:IAO_0000115>A district of Alfaro Ruiz Canton.</obo:IAO_0000115>
        <oboInOwl:hasOBONamespace>GAZ</oboInOwl:hasOBONamespace>
        <oboInOwl:id>GAZ:00118960</oboInOwl:id>
        <rdfs:label>Tapezco District</rdfs:label>
    </owl:NamedIndividual>
    


    <!-- http://purl.obolibrary.org/obo/GAZ_00118961 -->

    <owl:NamedIndividual rdf:about="http://purl.obolibrary.org/obo/GAZ_00118961">
        <rdf:type rdf:resource="http://purl.obolibrary.org/obo/ENVO_00000004"/>
        <obo:RO_0001025 rdf:resource="http://purl.obolibrary.org/obo/GAZ_00068659"/>
        <obo:IAO_0000115>A district of Alfaro Ruiz Canton.</obo:IAO_0000115>
        <oboInOwl:hasOBONamespace>GAZ</oboInOwl:hasOBONamespace>
        <oboInOwl:id>GAZ:00118961</oboInOwl:id>
        <rdfs:label>Brisas District</rdfs:label>
    </owl:NamedIndividual>
    


    <!-- http://purl.obolibrary.org/obo/GAZ_00118962 -->

    <owl:NamedIndividual rdf:about="http://purl.obolibrary.org/obo/GAZ_00118962">
        <rdf:type rdf:resource="http://purl.obolibrary.org/obo/ENVO_00000004"/>
        <obo:RO_0001025 rdf:resource="http://purl.obolibrary.org/obo/GAZ_00068653"/>
        <obo:IAO_0000115>A district of Valverde Vega Canton.</obo:IAO_0000115>
        <oboInOwl:hasOBONamespace>GAZ</oboInOwl:hasOBONamespace>
        <oboInOwl:id>GAZ:00118962</oboInOwl:id>
        <rdfs:label>Toro Amarillo District</rdfs:label>
    </owl:NamedIndividual>
    


    <!-- http://purl.obolibrary.org/obo/GAZ_00118963 -->

    <owl:NamedIndividual rdf:about="http://purl.obolibrary.org/obo/GAZ_00118963">
        <rdf:type rdf:resource="http://purl.obolibrary.org/obo/ENVO_00000004"/>
        <obo:RO_0001025 rdf:resource="http://purl.obolibrary.org/obo/GAZ_00068653"/>
        <obo:IAO_0000115>A district of Valverde Vega Canton.</obo:IAO_0000115>
        <oboInOwl:hasOBONamespace>GAZ</oboInOwl:hasOBONamespace>
        <oboInOwl:id>GAZ:00118963</oboInOwl:id>
        <rdfs:label>Sarchi Sur District</rdfs:label>
    </owl:NamedIndividual>
    


    <!-- http://purl.obolibrary.org/obo/GAZ_00118964 -->

    <owl:NamedIndividual rdf:about="http://purl.obolibrary.org/obo/GAZ_00118964">
        <rdf:type rdf:resource="http://purl.obolibrary.org/obo/ENVO_00000004"/>
        <obo:RO_0001025 rdf:resource="http://purl.obolibrary.org/obo/GAZ_00068653"/>
        <obo:IAO_0000115>A district of Valverde Vega Canton.</obo:IAO_0000115>
        <oboInOwl:hasOBONamespace>GAZ</oboInOwl:hasOBONamespace>
        <oboInOwl:id>GAZ:00118964</oboInOwl:id>
        <rdfs:label>Sarchi Norte District</rdfs:label>
    </owl:NamedIndividual>
    


    <!-- http://purl.obolibrary.org/obo/GAZ_00118965 -->

    <owl:NamedIndividual rdf:about="http://purl.obolibrary.org/obo/GAZ_00118965">
        <rdf:type rdf:resource="http://purl.obolibrary.org/obo/ENVO_00000004"/>
        <obo:RO_0001025 rdf:resource="http://purl.obolibrary.org/obo/GAZ_00068653"/>
        <obo:IAO_0000115>A district of Valverde Vega Canton.</obo:IAO_0000115>
        <oboInOwl:hasOBONamespace>GAZ</oboInOwl:hasOBONamespace>
        <oboInOwl:id>GAZ:00118965</oboInOwl:id>
        <rdfs:label>San Pedro District</rdfs:label>
    </owl:NamedIndividual>
    


    <!-- http://purl.obolibrary.org/obo/GAZ_00118966 -->

    <owl:NamedIndividual rdf:about="http://purl.obolibrary.org/obo/GAZ_00118966">
        <rdf:type rdf:resource="http://purl.obolibrary.org/obo/ENVO_00000004"/>
        <obo:RO_0001025 rdf:resource="http://purl.obolibrary.org/obo/GAZ_00068653"/>
        <obo:IAO_0000115>A district of Valverde Vega Canton.</obo:IAO_0000115>
        <oboInOwl:hasOBONamespace>GAZ</oboInOwl:hasOBONamespace>
        <oboInOwl:id>GAZ:00118966</oboInOwl:id>
        <rdfs:label>Rodriguez District</rdfs:label>
    </owl:NamedIndividual>
    


    <!-- http://purl.obolibrary.org/obo/GAZ_00118967 -->

    <owl:NamedIndividual rdf:about="http://purl.obolibrary.org/obo/GAZ_00118967">
        <rdf:type rdf:resource="http://purl.obolibrary.org/obo/ENVO_00000004"/>
        <obo:RO_0001025 rdf:resource="http://purl.obolibrary.org/obo/GAZ_00068647"/>
        <obo:IAO_0000115>A district of Los Chiles Canton.</obo:IAO_0000115>
        <oboInOwl:hasOBONamespace>GAZ</oboInOwl:hasOBONamespace>
        <oboInOwl:id>GAZ:00118967</oboInOwl:id>
        <rdfs:label>El Amparo District</rdfs:label>
    </owl:NamedIndividual>
    


    <!-- http://purl.obolibrary.org/obo/GAZ_00118968 -->

    <owl:NamedIndividual rdf:about="http://purl.obolibrary.org/obo/GAZ_00118968">
        <rdf:type rdf:resource="http://purl.obolibrary.org/obo/ENVO_00000004"/>
        <obo:RO_0001025 rdf:resource="http://purl.obolibrary.org/obo/GAZ_00068647"/>
        <obo:IAO_0000115>A district of Los Chiles Canton.</obo:IAO_0000115>
        <oboInOwl:hasOBONamespace>GAZ</oboInOwl:hasOBONamespace>
        <oboInOwl:id>GAZ:00118968</oboInOwl:id>
        <rdfs:label>Los Chiles District</rdfs:label>
    </owl:NamedIndividual>
    


    <!-- http://purl.obolibrary.org/obo/GAZ_00118969 -->

    <owl:NamedIndividual rdf:about="http://purl.obolibrary.org/obo/GAZ_00118969">
        <rdf:type rdf:resource="http://purl.obolibrary.org/obo/ENVO_00000004"/>
        <obo:RO_0001025 rdf:resource="http://purl.obolibrary.org/obo/GAZ_00068647"/>
        <obo:IAO_0000115>A district of Los Chiles Canton.</obo:IAO_0000115>
        <oboInOwl:hasOBONamespace>GAZ</oboInOwl:hasOBONamespace>
        <oboInOwl:id>GAZ:00118969</oboInOwl:id>
        <rdfs:label>San Jorge District</rdfs:label>
    </owl:NamedIndividual>
    


    <!-- http://purl.obolibrary.org/obo/GAZ_00118970 -->

    <owl:NamedIndividual rdf:about="http://purl.obolibrary.org/obo/GAZ_00118970">
        <rdf:type rdf:resource="http://purl.obolibrary.org/obo/ENVO_00000004"/>
        <obo:RO_0001025 rdf:resource="http://purl.obolibrary.org/obo/GAZ_00068647"/>
        <obo:IAO_0000115>A district of Los Chiles Canton.</obo:IAO_0000115>
        <oboInOwl:hasOBONamespace>GAZ</oboInOwl:hasOBONamespace>
        <oboInOwl:id>GAZ:00118970</oboInOwl:id>
        <rdfs:label>Cano Negro District</rdfs:label>
    </owl:NamedIndividual>
    


    <!-- http://purl.obolibrary.org/obo/GAZ_00118971 -->

    <owl:NamedIndividual rdf:about="http://purl.obolibrary.org/obo/GAZ_00118971">
        <rdf:type rdf:resource="http://purl.obolibrary.org/obo/ENVO_00000004"/>
        <obo:RO_0001025 rdf:resource="http://purl.obolibrary.org/obo/GAZ_00068649"/>
        <obo:IAO_0000115>A district of Guatuso Canton.</obo:IAO_0000115>
        <oboInOwl:hasOBONamespace>GAZ</oboInOwl:hasOBONamespace>
        <oboInOwl:id>GAZ:00118971</oboInOwl:id>
        <rdfs:label>Cote District</rdfs:label>
    </owl:NamedIndividual>
    


    <!-- http://purl.obolibrary.org/obo/GAZ_00118972 -->

    <owl:NamedIndividual rdf:about="http://purl.obolibrary.org/obo/GAZ_00118972">
        <rdf:type rdf:resource="http://purl.obolibrary.org/obo/ENVO_00000004"/>
        <obo:RO_0001025 rdf:resource="http://purl.obolibrary.org/obo/GAZ_00068649"/>
        <obo:IAO_0000115>A district of Guatuso Canton.</obo:IAO_0000115>
        <oboInOwl:hasOBONamespace>GAZ</oboInOwl:hasOBONamespace>
        <oboInOwl:id>GAZ:00118972</oboInOwl:id>
        <rdfs:label>Buenavista District</rdfs:label>
    </owl:NamedIndividual>
    


    <!-- http://purl.obolibrary.org/obo/GAZ_00118973 -->

    <owl:NamedIndividual rdf:about="http://purl.obolibrary.org/obo/GAZ_00118973">
        <rdf:type rdf:resource="http://purl.obolibrary.org/obo/ENVO_00000004"/>
        <obo:RO_0001025 rdf:resource="http://purl.obolibrary.org/obo/GAZ_00068649"/>
        <obo:IAO_0000115>A district of Guatuso Canton.</obo:IAO_0000115>
        <oboInOwl:hasOBONamespace>GAZ</oboInOwl:hasOBONamespace>
        <oboInOwl:id>GAZ:00118973</oboInOwl:id>
        <rdfs:label>San Rafael District</rdfs:label>
    </owl:NamedIndividual>
    


    <!-- http://purl.obolibrary.org/obo/GAZ_00118974 -->

    <owl:NamedIndividual rdf:about="http://purl.obolibrary.org/obo/GAZ_00118974">
        <rdf:type rdf:resource="http://purl.obolibrary.org/obo/ENVO_00000004"/>
        <obo:RO_0001025 rdf:resource="http://purl.obolibrary.org/obo/GAZ_00068663"/>
        <obo:IAO_0000115>A district of Alvarado Canton.</obo:IAO_0000115>
        <oboInOwl:hasOBONamespace>GAZ</oboInOwl:hasOBONamespace>
        <oboInOwl:id>GAZ:00118974</oboInOwl:id>
        <rdfs:label>Capellades District</rdfs:label>
    </owl:NamedIndividual>
    


    <!-- http://purl.obolibrary.org/obo/GAZ_00118975 -->

    <owl:NamedIndividual rdf:about="http://purl.obolibrary.org/obo/GAZ_00118975">
        <rdf:type rdf:resource="http://purl.obolibrary.org/obo/ENVO_00000004"/>
        <obo:RO_0001025 rdf:resource="http://purl.obolibrary.org/obo/GAZ_00068663"/>
        <obo:IAO_0000115>A district of Alvarado Canton.</obo:IAO_0000115>
        <oboInOwl:hasOBONamespace>GAZ</oboInOwl:hasOBONamespace>
        <oboInOwl:id>GAZ:00118975</oboInOwl:id>
        <rdfs:label>Pacayas District</rdfs:label>
    </owl:NamedIndividual>
    


    <!-- http://purl.obolibrary.org/obo/GAZ_00118976 -->

    <owl:NamedIndividual rdf:about="http://purl.obolibrary.org/obo/GAZ_00118976">
        <rdf:type rdf:resource="http://purl.obolibrary.org/obo/ENVO_00000004"/>
        <obo:RO_0001025 rdf:resource="http://purl.obolibrary.org/obo/GAZ_00068663"/>
        <obo:IAO_0000115>A district of Alvarado Canton.</obo:IAO_0000115>
        <oboInOwl:hasOBONamespace>GAZ</oboInOwl:hasOBONamespace>
        <oboInOwl:id>GAZ:00118976</oboInOwl:id>
        <rdfs:label>Cervantes District</rdfs:label>
    </owl:NamedIndividual>
    


    <!-- http://purl.obolibrary.org/obo/GAZ_00118977 -->

    <owl:NamedIndividual rdf:about="http://purl.obolibrary.org/obo/GAZ_00118977">
        <rdf:type rdf:resource="http://purl.obolibrary.org/obo/ENVO_00000004"/>
        <obo:RO_0001025 rdf:resource="http://purl.obolibrary.org/obo/GAZ_00068667"/>
        <obo:IAO_0000115>A district of Paraiso Canton.</obo:IAO_0000115>
        <oboInOwl:hasOBONamespace>GAZ</oboInOwl:hasOBONamespace>
        <oboInOwl:id>GAZ:00118977</oboInOwl:id>
        <rdfs:label>Paraiso District</rdfs:label>
    </owl:NamedIndividual>
    


    <!-- http://purl.obolibrary.org/obo/GAZ_00118978 -->

    <owl:NamedIndividual rdf:about="http://purl.obolibrary.org/obo/GAZ_00118978">
        <rdf:type rdf:resource="http://purl.obolibrary.org/obo/ENVO_00000004"/>
        <obo:RO_0001025 rdf:resource="http://purl.obolibrary.org/obo/GAZ_00068667"/>
        <obo:IAO_0000115>A district of Paraiso Canton.</obo:IAO_0000115>
        <oboInOwl:hasOBONamespace>GAZ</oboInOwl:hasOBONamespace>
        <oboInOwl:id>GAZ:00118978</oboInOwl:id>
        <rdfs:label>Santiago District</rdfs:label>
    </owl:NamedIndividual>
    


    <!-- http://purl.obolibrary.org/obo/GAZ_00118979 -->

    <owl:NamedIndividual rdf:about="http://purl.obolibrary.org/obo/GAZ_00118979">
        <rdf:type rdf:resource="http://purl.obolibrary.org/obo/ENVO_00000004"/>
        <obo:RO_0001025 rdf:resource="http://purl.obolibrary.org/obo/GAZ_00068667"/>
        <obo:IAO_0000115>A district of Paraiso Canton.</obo:IAO_0000115>
        <oboInOwl:hasOBONamespace>GAZ</oboInOwl:hasOBONamespace>
        <oboInOwl:id>GAZ:00118979</oboInOwl:id>
        <rdfs:label>Orosi District</rdfs:label>
    </owl:NamedIndividual>
    


    <!-- http://purl.obolibrary.org/obo/GAZ_00118980 -->

    <owl:NamedIndividual rdf:about="http://purl.obolibrary.org/obo/GAZ_00118980">
        <rdf:type rdf:resource="http://purl.obolibrary.org/obo/ENVO_00000004"/>
        <obo:RO_0001025 rdf:resource="http://purl.obolibrary.org/obo/GAZ_00068667"/>
        <obo:IAO_0000115>A district of Paraiso Canton.</obo:IAO_0000115>
        <oboInOwl:hasOBONamespace>GAZ</oboInOwl:hasOBONamespace>
        <oboInOwl:id>GAZ:00118980</oboInOwl:id>
        <rdfs:label>Cachi District</rdfs:label>
    </owl:NamedIndividual>
    


    <!-- http://purl.obolibrary.org/obo/GAZ_00118981 -->

    <owl:NamedIndividual rdf:about="http://purl.obolibrary.org/obo/GAZ_00118981">
        <rdf:type rdf:resource="http://purl.obolibrary.org/obo/ENVO_00000004"/>
        <obo:RO_0001025 rdf:resource="http://purl.obolibrary.org/obo/GAZ_00068667"/>
        <obo:IAO_0000115>A district of Paraiso Canton.</obo:IAO_0000115>
        <oboInOwl:hasOBONamespace>GAZ</oboInOwl:hasOBONamespace>
        <oboInOwl:id>GAZ:00118981</oboInOwl:id>
        <rdfs:label>Santa Lucia District</rdfs:label>
    </owl:NamedIndividual>
    


    <!-- http://purl.obolibrary.org/obo/GAZ_00118982 -->

    <owl:NamedIndividual rdf:about="http://purl.obolibrary.org/obo/GAZ_00118982">
        <rdf:type rdf:resource="http://purl.obolibrary.org/obo/ENVO_00000004"/>
        <obo:RO_0001025 rdf:resource="http://purl.obolibrary.org/obo/GAZ_00068665"/>
        <obo:IAO_0000115>A district of La Union Canton.</obo:IAO_0000115>
        <oboInOwl:hasOBONamespace>GAZ</oboInOwl:hasOBONamespace>
        <oboInOwl:id>GAZ:00118982</oboInOwl:id>
        <rdfs:label>San Rafael District</rdfs:label>
    </owl:NamedIndividual>
    


    <!-- http://purl.obolibrary.org/obo/GAZ_00118983 -->

    <owl:NamedIndividual rdf:about="http://purl.obolibrary.org/obo/GAZ_00118983">
        <rdf:type rdf:resource="http://purl.obolibrary.org/obo/ENVO_00000004"/>
        <obo:RO_0001025 rdf:resource="http://purl.obolibrary.org/obo/GAZ_00068665"/>
        <obo:IAO_0000115>A district of La Union Canton.</obo:IAO_0000115>
        <oboInOwl:hasOBONamespace>GAZ</oboInOwl:hasOBONamespace>
        <oboInOwl:id>GAZ:00118983</oboInOwl:id>
        <rdfs:label>Dulce Nombre District</rdfs:label>
    </owl:NamedIndividual>
    


    <!-- http://purl.obolibrary.org/obo/GAZ_00118984 -->

    <owl:NamedIndividual rdf:about="http://purl.obolibrary.org/obo/GAZ_00118984">
        <rdf:type rdf:resource="http://purl.obolibrary.org/obo/ENVO_00000004"/>
        <obo:RO_0001025 rdf:resource="http://purl.obolibrary.org/obo/GAZ_00068665"/>
        <obo:IAO_0000115>A district of La Union Canton.</obo:IAO_0000115>
        <oboInOwl:hasOBONamespace>GAZ</oboInOwl:hasOBONamespace>
        <oboInOwl:id>GAZ:00118984</oboInOwl:id>
        <rdfs:label>Rio Azul District</rdfs:label>
    </owl:NamedIndividual>
    


    <!-- http://purl.obolibrary.org/obo/GAZ_00118985 -->

    <owl:NamedIndividual rdf:about="http://purl.obolibrary.org/obo/GAZ_00118985">
        <rdf:type rdf:resource="http://purl.obolibrary.org/obo/ENVO_00000004"/>
        <obo:RO_0001025 rdf:resource="http://purl.obolibrary.org/obo/GAZ_00068665"/>
        <obo:IAO_0000115>A district of La Union Canton.</obo:IAO_0000115>
        <oboInOwl:hasOBONamespace>GAZ</oboInOwl:hasOBONamespace>
        <oboInOwl:id>GAZ:00118985</oboInOwl:id>
        <rdfs:label>Concepcion District</rdfs:label>
    </owl:NamedIndividual>
    


    <!-- http://purl.obolibrary.org/obo/GAZ_00118986 -->

    <owl:NamedIndividual rdf:about="http://purl.obolibrary.org/obo/GAZ_00118986">
        <rdf:type rdf:resource="http://purl.obolibrary.org/obo/ENVO_00000004"/>
        <obo:RO_0001025 rdf:resource="http://purl.obolibrary.org/obo/GAZ_00068665"/>
        <obo:IAO_0000115>A district of La Union Canton.</obo:IAO_0000115>
        <oboInOwl:hasOBONamespace>GAZ</oboInOwl:hasOBONamespace>
        <oboInOwl:id>GAZ:00118986</oboInOwl:id>
        <rdfs:label>San Ramon District</rdfs:label>
    </owl:NamedIndividual>
    


    <!-- http://purl.obolibrary.org/obo/GAZ_00118987 -->

    <owl:NamedIndividual rdf:about="http://purl.obolibrary.org/obo/GAZ_00118987">
        <rdf:type rdf:resource="http://purl.obolibrary.org/obo/ENVO_00000004"/>
        <obo:RO_0001025 rdf:resource="http://purl.obolibrary.org/obo/GAZ_00068665"/>
        <obo:IAO_0000115>A district of La Union Canton.</obo:IAO_0000115>
        <oboInOwl:hasOBONamespace>GAZ</oboInOwl:hasOBONamespace>
        <oboInOwl:id>GAZ:00118987</oboInOwl:id>
        <rdfs:label>San Juan District</rdfs:label>
    </owl:NamedIndividual>
    


    <!-- http://purl.obolibrary.org/obo/GAZ_00118988 -->

    <owl:NamedIndividual rdf:about="http://purl.obolibrary.org/obo/GAZ_00118988">
        <rdf:type rdf:resource="http://purl.obolibrary.org/obo/ENVO_00000004"/>
        <obo:RO_0001025 rdf:resource="http://purl.obolibrary.org/obo/GAZ_00068665"/>
        <obo:IAO_0000115>A district of La Union Canton.</obo:IAO_0000115>
        <oboInOwl:hasOBONamespace>GAZ</oboInOwl:hasOBONamespace>
        <oboInOwl:id>GAZ:00118988</oboInOwl:id>
        <rdfs:label>San Diego District</rdfs:label>
    </owl:NamedIndividual>
    


    <!-- http://purl.obolibrary.org/obo/GAZ_00118989 -->

    <owl:NamedIndividual rdf:about="http://purl.obolibrary.org/obo/GAZ_00118989">
        <rdf:type rdf:resource="http://purl.obolibrary.org/obo/ENVO_00000004"/>
        <obo:RO_0001025 rdf:resource="http://purl.obolibrary.org/obo/GAZ_00068665"/>
        <obo:IAO_0000115>A district of La Union Canton.</obo:IAO_0000115>
        <oboInOwl:hasOBONamespace>GAZ</oboInOwl:hasOBONamespace>
        <oboInOwl:id>GAZ:00118989</oboInOwl:id>
        <rdfs:label>Tres Rios District</rdfs:label>
    </owl:NamedIndividual>
    


    <!-- http://purl.obolibrary.org/obo/GAZ_00118990 -->

    <owl:NamedIndividual rdf:about="http://purl.obolibrary.org/obo/GAZ_00118990">
        <rdf:type rdf:resource="http://purl.obolibrary.org/obo/ENVO_00000004"/>
        <obo:RO_0001025 rdf:resource="http://purl.obolibrary.org/obo/GAZ_00068662"/>
        <obo:IAO_0000115>A district of Jimenez Canton.</obo:IAO_0000115>
        <oboInOwl:hasOBONamespace>GAZ</oboInOwl:hasOBONamespace>
        <oboInOwl:id>GAZ:00118990</oboInOwl:id>
        <rdfs:label>Juan Vinas District</rdfs:label>
    </owl:NamedIndividual>
    


    <!-- http://purl.obolibrary.org/obo/GAZ_00118991 -->

    <owl:NamedIndividual rdf:about="http://purl.obolibrary.org/obo/GAZ_00118991">
        <rdf:type rdf:resource="http://purl.obolibrary.org/obo/ENVO_00000004"/>
        <obo:RO_0001025 rdf:resource="http://purl.obolibrary.org/obo/GAZ_00068662"/>
        <obo:IAO_0000115>A district of Jimenez Canton.</obo:IAO_0000115>
        <oboInOwl:hasOBONamespace>GAZ</oboInOwl:hasOBONamespace>
        <oboInOwl:id>GAZ:00118991</oboInOwl:id>
        <rdfs:label>Pejibaye District</rdfs:label>
    </owl:NamedIndividual>
    


    <!-- http://purl.obolibrary.org/obo/GAZ_00118992 -->

    <owl:NamedIndividual rdf:about="http://purl.obolibrary.org/obo/GAZ_00118992">
        <rdf:type rdf:resource="http://purl.obolibrary.org/obo/ENVO_00000004"/>
        <obo:RO_0001025 rdf:resource="http://purl.obolibrary.org/obo/GAZ_00068662"/>
        <obo:IAO_0000115>A district of Jimenez Canton.</obo:IAO_0000115>
        <oboInOwl:hasOBONamespace>GAZ</oboInOwl:hasOBONamespace>
        <oboInOwl:id>GAZ:00118992</oboInOwl:id>
        <rdfs:label>Tucurrique District</rdfs:label>
    </owl:NamedIndividual>
    


    <!-- http://purl.obolibrary.org/obo/GAZ_00118993 -->

    <owl:NamedIndividual rdf:about="http://purl.obolibrary.org/obo/GAZ_00118993">
        <rdf:type rdf:resource="http://purl.obolibrary.org/obo/ENVO_00000004"/>
        <obo:RO_0001025 rdf:resource="http://purl.obolibrary.org/obo/GAZ_00009455"/>
        <obo:IAO_0000115>A district of Turrialba Canton.</obo:IAO_0000115>
        <oboInOwl:hasOBONamespace>GAZ</oboInOwl:hasOBONamespace>
        <oboInOwl:id>GAZ:00118993</oboInOwl:id>
        <rdfs:label>Tuis District</rdfs:label>
    </owl:NamedIndividual>
    


    <!-- http://purl.obolibrary.org/obo/GAZ_00118994 -->

    <owl:NamedIndividual rdf:about="http://purl.obolibrary.org/obo/GAZ_00118994">
        <rdf:type rdf:resource="http://purl.obolibrary.org/obo/ENVO_00000004"/>
        <obo:RO_0001025 rdf:resource="http://purl.obolibrary.org/obo/GAZ_00009455"/>
        <obo:IAO_0000115>A district of Turrialba Canton.</obo:IAO_0000115>
        <oboInOwl:hasOBONamespace>GAZ</oboInOwl:hasOBONamespace>
        <oboInOwl:id>GAZ:00118994</oboInOwl:id>
        <rdfs:label>Turrialba District</rdfs:label>
    </owl:NamedIndividual>
    


    <!-- http://purl.obolibrary.org/obo/GAZ_00118995 -->

    <owl:NamedIndividual rdf:about="http://purl.obolibrary.org/obo/GAZ_00118995">
        <rdf:type rdf:resource="http://purl.obolibrary.org/obo/ENVO_00000004"/>
        <obo:RO_0001025 rdf:resource="http://purl.obolibrary.org/obo/GAZ_00009455"/>
        <obo:IAO_0000115>A district of Turrialba Canton.</obo:IAO_0000115>
        <oboInOwl:hasOBONamespace>GAZ</oboInOwl:hasOBONamespace>
        <oboInOwl:id>GAZ:00118995</oboInOwl:id>
        <rdfs:label>Pavones District</rdfs:label>
    </owl:NamedIndividual>
    


    <!-- http://purl.obolibrary.org/obo/GAZ_00118996 -->

    <owl:NamedIndividual rdf:about="http://purl.obolibrary.org/obo/GAZ_00118996">
        <rdf:type rdf:resource="http://purl.obolibrary.org/obo/ENVO_00000004"/>
        <obo:RO_0001025 rdf:resource="http://purl.obolibrary.org/obo/GAZ_00009455"/>
        <obo:IAO_0000115>A district of Turrialba Canton.</obo:IAO_0000115>
        <oboInOwl:hasOBONamespace>GAZ</oboInOwl:hasOBONamespace>
        <oboInOwl:id>GAZ:00118996</oboInOwl:id>
        <rdfs:label>Tres Equis District</rdfs:label>
    </owl:NamedIndividual>
    


    <!-- http://purl.obolibrary.org/obo/GAZ_00118997 -->

    <owl:NamedIndividual rdf:about="http://purl.obolibrary.org/obo/GAZ_00118997">
        <rdf:type rdf:resource="http://purl.obolibrary.org/obo/ENVO_00000004"/>
        <obo:RO_0001025 rdf:resource="http://purl.obolibrary.org/obo/GAZ_00009455"/>
        <obo:IAO_0000115>A district of Turrialba Canton.</obo:IAO_0000115>
        <oboInOwl:hasOBONamespace>GAZ</oboInOwl:hasOBONamespace>
        <oboInOwl:id>GAZ:00118997</oboInOwl:id>
        <rdfs:label>La Suiza District</rdfs:label>
    </owl:NamedIndividual>
    


    <!-- http://purl.obolibrary.org/obo/GAZ_00118998 -->

    <owl:NamedIndividual rdf:about="http://purl.obolibrary.org/obo/GAZ_00118998">
        <rdf:type rdf:resource="http://purl.obolibrary.org/obo/ENVO_00000004"/>
        <obo:RO_0001025 rdf:resource="http://purl.obolibrary.org/obo/GAZ_00009455"/>
        <obo:IAO_0000115>A district of Turrialba Canton.</obo:IAO_0000115>
        <oboInOwl:hasOBONamespace>GAZ</oboInOwl:hasOBONamespace>
        <oboInOwl:id>GAZ:00118998</oboInOwl:id>
        <rdfs:label>Santa Cruz District</rdfs:label>
    </owl:NamedIndividual>
    


    <!-- http://purl.obolibrary.org/obo/GAZ_00118999 -->

    <owl:NamedIndividual rdf:about="http://purl.obolibrary.org/obo/GAZ_00118999">
        <rdf:type rdf:resource="http://purl.obolibrary.org/obo/ENVO_00000004"/>
        <obo:RO_0001025 rdf:resource="http://purl.obolibrary.org/obo/GAZ_00009455"/>
        <obo:IAO_0000115>A district of Turrialba Canton.</obo:IAO_0000115>
        <oboInOwl:hasOBONamespace>GAZ</oboInOwl:hasOBONamespace>
        <oboInOwl:id>GAZ:00118999</oboInOwl:id>
        <rdfs:label>Santa Rosa District</rdfs:label>
    </owl:NamedIndividual>
    


    <!-- http://purl.obolibrary.org/obo/GAZ_00119000 -->

    <owl:NamedIndividual rdf:about="http://purl.obolibrary.org/obo/GAZ_00119000">
        <rdf:type rdf:resource="http://purl.obolibrary.org/obo/ENVO_00000004"/>
        <obo:RO_0001025 rdf:resource="http://purl.obolibrary.org/obo/GAZ_00009455"/>
        <obo:IAO_0000115>A district of Turrialba Canton.</obo:IAO_0000115>
        <oboInOwl:hasOBONamespace>GAZ</oboInOwl:hasOBONamespace>
        <oboInOwl:id>GAZ:00119000</oboInOwl:id>
        <rdfs:label>Tayutic District</rdfs:label>
    </owl:NamedIndividual>
    


    <!-- http://purl.obolibrary.org/obo/GAZ_00119001 -->

    <owl:NamedIndividual rdf:about="http://purl.obolibrary.org/obo/GAZ_00119001">
        <rdf:type rdf:resource="http://purl.obolibrary.org/obo/ENVO_00000004"/>
        <obo:RO_0001025 rdf:resource="http://purl.obolibrary.org/obo/GAZ_00009455"/>
        <obo:IAO_0000115>A district of Turrialba Canton.</obo:IAO_0000115>
        <oboInOwl:hasOBONamespace>GAZ</oboInOwl:hasOBONamespace>
        <oboInOwl:id>GAZ:00119001</oboInOwl:id>
        <rdfs:label>Peralta District</rdfs:label>
    </owl:NamedIndividual>
    


    <!-- http://purl.obolibrary.org/obo/GAZ_00119002 -->

    <owl:NamedIndividual rdf:about="http://purl.obolibrary.org/obo/GAZ_00119002">
        <rdf:type rdf:resource="http://purl.obolibrary.org/obo/ENVO_00000004"/>
        <obo:RO_0001025 rdf:resource="http://purl.obolibrary.org/obo/GAZ_00009455"/>
        <obo:IAO_0000115>A district of Turrialba Canton.</obo:IAO_0000115>
        <oboInOwl:hasOBONamespace>GAZ</oboInOwl:hasOBONamespace>
        <oboInOwl:id>GAZ:00119002</oboInOwl:id>
        <rdfs:label>Santa Teresita District</rdfs:label>
    </owl:NamedIndividual>
    


    <!-- http://purl.obolibrary.org/obo/GAZ_00119003 -->

    <owl:NamedIndividual rdf:about="http://purl.obolibrary.org/obo/GAZ_00119003">
        <rdf:type rdf:resource="http://purl.obolibrary.org/obo/ENVO_00000004"/>
        <obo:RO_0001025 rdf:resource="http://purl.obolibrary.org/obo/GAZ_00068668"/>
        <obo:IAO_0000115>A district of Oreamuno Canton.</obo:IAO_0000115>
        <oboInOwl:hasOBONamespace>GAZ</oboInOwl:hasOBONamespace>
        <oboInOwl:id>GAZ:00119003</oboInOwl:id>
        <rdfs:label>Santa Rosa District</rdfs:label>
    </owl:NamedIndividual>
    


    <!-- http://purl.obolibrary.org/obo/GAZ_00119004 -->

    <owl:NamedIndividual rdf:about="http://purl.obolibrary.org/obo/GAZ_00119004">
        <rdf:type rdf:resource="http://purl.obolibrary.org/obo/ENVO_00000004"/>
        <obo:RO_0001025 rdf:resource="http://purl.obolibrary.org/obo/GAZ_00068668"/>
        <obo:IAO_0000115>A district of Oreamuno Canton.</obo:IAO_0000115>
        <oboInOwl:hasOBONamespace>GAZ</oboInOwl:hasOBONamespace>
        <oboInOwl:id>GAZ:00119004</oboInOwl:id>
        <rdfs:label>San Rafael District</rdfs:label>
    </owl:NamedIndividual>
    


    <!-- http://purl.obolibrary.org/obo/GAZ_00119005 -->

    <owl:NamedIndividual rdf:about="http://purl.obolibrary.org/obo/GAZ_00119005">
        <rdf:type rdf:resource="http://purl.obolibrary.org/obo/ENVO_00000004"/>
        <obo:RO_0001025 rdf:resource="http://purl.obolibrary.org/obo/GAZ_00068668"/>
        <obo:IAO_0000115>A district of Oreamuno Canton.</obo:IAO_0000115>
        <oboInOwl:hasOBONamespace>GAZ</oboInOwl:hasOBONamespace>
        <oboInOwl:id>GAZ:00119005</oboInOwl:id>
        <rdfs:label>Cipreses District</rdfs:label>
    </owl:NamedIndividual>
    


    <!-- http://purl.obolibrary.org/obo/GAZ_00119006 -->

    <owl:NamedIndividual rdf:about="http://purl.obolibrary.org/obo/GAZ_00119006">
        <rdf:type rdf:resource="http://purl.obolibrary.org/obo/ENVO_00000004"/>
        <obo:RO_0001025 rdf:resource="http://purl.obolibrary.org/obo/GAZ_00068668"/>
        <obo:IAO_0000115>A district of Oreamuno Canton.</obo:IAO_0000115>
        <oboInOwl:hasOBONamespace>GAZ</oboInOwl:hasOBONamespace>
        <oboInOwl:id>GAZ:00119006</oboInOwl:id>
        <rdfs:label>Potrero Cerrado District</rdfs:label>
    </owl:NamedIndividual>
    


    <!-- http://purl.obolibrary.org/obo/GAZ_00119007 -->

    <owl:NamedIndividual rdf:about="http://purl.obolibrary.org/obo/GAZ_00119007">
        <rdf:type rdf:resource="http://purl.obolibrary.org/obo/ENVO_00000004"/>
        <obo:RO_0001025 rdf:resource="http://purl.obolibrary.org/obo/GAZ_00068668"/>
        <obo:IAO_0000115>A district of Oreamuno Canton.</obo:IAO_0000115>
        <oboInOwl:hasOBONamespace>GAZ</oboInOwl:hasOBONamespace>
        <oboInOwl:id>GAZ:00119007</oboInOwl:id>
        <rdfs:label>Cot District</rdfs:label>
    </owl:NamedIndividual>
    


    <!-- http://purl.obolibrary.org/obo/GAZ_00119008 -->

    <owl:NamedIndividual rdf:about="http://purl.obolibrary.org/obo/GAZ_00119008">
        <rdf:type rdf:resource="http://purl.obolibrary.org/obo/ENVO_00000004"/>
        <obo:RO_0001025 rdf:resource="http://purl.obolibrary.org/obo/GAZ_00068666"/>
        <obo:IAO_0000115>A district of Cartago Canton.</obo:IAO_0000115>
        <oboInOwl:hasOBONamespace>GAZ</oboInOwl:hasOBONamespace>
        <oboInOwl:id>GAZ:00119008</oboInOwl:id>
        <rdfs:label>Guadalupe District</rdfs:label>
    </owl:NamedIndividual>
    


    <!-- http://purl.obolibrary.org/obo/GAZ_00119009 -->

    <owl:NamedIndividual rdf:about="http://purl.obolibrary.org/obo/GAZ_00119009">
        <rdf:type rdf:resource="http://purl.obolibrary.org/obo/ENVO_00000004"/>
        <obo:RO_0001025 rdf:resource="http://purl.obolibrary.org/obo/GAZ_00068666"/>
        <obo:IAO_0000115>A district of Cartago Canton.</obo:IAO_0000115>
        <oboInOwl:hasOBONamespace>GAZ</oboInOwl:hasOBONamespace>
        <oboInOwl:id>GAZ:00119009</oboInOwl:id>
        <rdfs:label>Corralillo District</rdfs:label>
    </owl:NamedIndividual>
    


    <!-- http://purl.obolibrary.org/obo/GAZ_00119010 -->

    <owl:NamedIndividual rdf:about="http://purl.obolibrary.org/obo/GAZ_00119010">
        <rdf:type rdf:resource="http://purl.obolibrary.org/obo/ENVO_00000004"/>
        <obo:RO_0001025 rdf:resource="http://purl.obolibrary.org/obo/GAZ_00068666"/>
        <obo:IAO_0000115>A district of Cartago Canton.</obo:IAO_0000115>
        <oboInOwl:hasOBONamespace>GAZ</oboInOwl:hasOBONamespace>
        <oboInOwl:id>GAZ:00119010</oboInOwl:id>
        <rdfs:label>San Nicolas District</rdfs:label>
    </owl:NamedIndividual>
    


    <!-- http://purl.obolibrary.org/obo/GAZ_00119011 -->

    <owl:NamedIndividual rdf:about="http://purl.obolibrary.org/obo/GAZ_00119011">
        <rdf:type rdf:resource="http://purl.obolibrary.org/obo/ENVO_00000004"/>
        <obo:RO_0001025 rdf:resource="http://purl.obolibrary.org/obo/GAZ_00068666"/>
        <obo:IAO_0000115>A district of Cartago Canton.</obo:IAO_0000115>
        <oboInOwl:hasOBONamespace>GAZ</oboInOwl:hasOBONamespace>
        <oboInOwl:id>GAZ:00119011</oboInOwl:id>
        <rdfs:label>Occidental District</rdfs:label>
    </owl:NamedIndividual>
    


    <!-- http://purl.obolibrary.org/obo/GAZ_00119012 -->

    <owl:NamedIndividual rdf:about="http://purl.obolibrary.org/obo/GAZ_00119012">
        <rdf:type rdf:resource="http://purl.obolibrary.org/obo/ENVO_00000004"/>
        <obo:RO_0001025 rdf:resource="http://purl.obolibrary.org/obo/GAZ_00068666"/>
        <obo:IAO_0000115>A district of Cartago Canton.</obo:IAO_0000115>
        <oboInOwl:hasOBONamespace>GAZ</oboInOwl:hasOBONamespace>
        <oboInOwl:id>GAZ:00119012</oboInOwl:id>
        <rdfs:label>El Carmen District</rdfs:label>
    </owl:NamedIndividual>
    


    <!-- http://purl.obolibrary.org/obo/GAZ_00119013 -->

    <owl:NamedIndividual rdf:about="http://purl.obolibrary.org/obo/GAZ_00119013">
        <rdf:type rdf:resource="http://purl.obolibrary.org/obo/ENVO_00000004"/>
        <obo:RO_0001025 rdf:resource="http://purl.obolibrary.org/obo/GAZ_00068666"/>
        <obo:IAO_0000115>A district of Cartago Canton.</obo:IAO_0000115>
        <oboInOwl:hasOBONamespace>GAZ</oboInOwl:hasOBONamespace>
        <oboInOwl:id>GAZ:00119013</oboInOwl:id>
        <rdfs:label>Tierra Blanca District</rdfs:label>
    </owl:NamedIndividual>
    


    <!-- http://purl.obolibrary.org/obo/GAZ_00119014 -->

    <owl:NamedIndividual rdf:about="http://purl.obolibrary.org/obo/GAZ_00119014">
        <rdf:type rdf:resource="http://purl.obolibrary.org/obo/ENVO_00000004"/>
        <obo:RO_0001025 rdf:resource="http://purl.obolibrary.org/obo/GAZ_00068666"/>
        <obo:IAO_0000115>A district of Cartago Canton.</obo:IAO_0000115>
        <oboInOwl:hasOBONamespace>GAZ</oboInOwl:hasOBONamespace>
        <oboInOwl:id>GAZ:00119014</oboInOwl:id>
        <rdfs:label>Oriental District</rdfs:label>
    </owl:NamedIndividual>
    


    <!-- http://purl.obolibrary.org/obo/GAZ_00119015 -->

    <owl:NamedIndividual rdf:about="http://purl.obolibrary.org/obo/GAZ_00119015">
        <rdf:type rdf:resource="http://purl.obolibrary.org/obo/ENVO_00000004"/>
        <obo:RO_0001025 rdf:resource="http://purl.obolibrary.org/obo/GAZ_00068666"/>
        <obo:IAO_0000115>A district of Cartago Canton.</obo:IAO_0000115>
        <oboInOwl:hasOBONamespace>GAZ</oboInOwl:hasOBONamespace>
        <oboInOwl:id>GAZ:00119015</oboInOwl:id>
        <rdfs:label>Llano Grande District</rdfs:label>
    </owl:NamedIndividual>
    


    <!-- http://purl.obolibrary.org/obo/GAZ_00119016 -->

    <owl:NamedIndividual rdf:about="http://purl.obolibrary.org/obo/GAZ_00119016">
        <rdf:type rdf:resource="http://purl.obolibrary.org/obo/ENVO_00000004"/>
        <obo:RO_0001025 rdf:resource="http://purl.obolibrary.org/obo/GAZ_00068666"/>
        <obo:IAO_0000115>A district of Cartago Canton.</obo:IAO_0000115>
        <oboInOwl:hasOBONamespace>GAZ</oboInOwl:hasOBONamespace>
        <oboInOwl:id>GAZ:00119016</oboInOwl:id>
        <rdfs:label>Dulce Nombre District</rdfs:label>
    </owl:NamedIndividual>
    


    <!-- http://purl.obolibrary.org/obo/GAZ_00119017 -->

    <owl:NamedIndividual rdf:about="http://purl.obolibrary.org/obo/GAZ_00119017">
        <rdf:type rdf:resource="http://purl.obolibrary.org/obo/ENVO_00000004"/>
        <obo:RO_0001025 rdf:resource="http://purl.obolibrary.org/obo/GAZ_00068666"/>
        <obo:IAO_0000115>A district of Cartago Canton.</obo:IAO_0000115>
        <oboInOwl:hasOBONamespace>GAZ</oboInOwl:hasOBONamespace>
        <oboInOwl:id>GAZ:00119017</oboInOwl:id>
        <rdfs:label>Quebradilla District</rdfs:label>
    </owl:NamedIndividual>
    


    <!-- http://purl.obolibrary.org/obo/GAZ_00119018 -->

    <owl:NamedIndividual rdf:about="http://purl.obolibrary.org/obo/GAZ_00119018">
        <rdf:type rdf:resource="http://purl.obolibrary.org/obo/ENVO_00000004"/>
        <obo:RO_0001025 rdf:resource="http://purl.obolibrary.org/obo/GAZ_00068666"/>
        <obo:IAO_0000115>A district of Cartago Canton.</obo:IAO_0000115>
        <oboInOwl:hasOBONamespace>GAZ</oboInOwl:hasOBONamespace>
        <oboInOwl:id>GAZ:00119018</oboInOwl:id>
        <rdfs:label>San Francisco District</rdfs:label>
    </owl:NamedIndividual>
    


    <!-- http://purl.obolibrary.org/obo/GAZ_00119019 -->

    <owl:NamedIndividual rdf:about="http://purl.obolibrary.org/obo/GAZ_00119019">
        <rdf:type rdf:resource="http://purl.obolibrary.org/obo/ENVO_00000004"/>
        <obo:RO_0001025 rdf:resource="http://purl.obolibrary.org/obo/GAZ_00068664"/>
        <obo:IAO_0000115>A district of El Guarco Canton.</obo:IAO_0000115>
        <oboInOwl:hasOBONamespace>GAZ</oboInOwl:hasOBONamespace>
        <oboInOwl:id>GAZ:00119019</oboInOwl:id>
        <rdfs:label>San Isidro District</rdfs:label>
    </owl:NamedIndividual>
    


    <!-- http://purl.obolibrary.org/obo/GAZ_00119020 -->

    <owl:NamedIndividual rdf:about="http://purl.obolibrary.org/obo/GAZ_00119020">
        <rdf:type rdf:resource="http://purl.obolibrary.org/obo/ENVO_00000004"/>
        <obo:RO_0001025 rdf:resource="http://purl.obolibrary.org/obo/GAZ_00068664"/>
        <obo:IAO_0000115>A district of El Guarco Canton.</obo:IAO_0000115>
        <oboInOwl:hasOBONamespace>GAZ</oboInOwl:hasOBONamespace>
        <oboInOwl:id>GAZ:00119020</oboInOwl:id>
        <rdfs:label>Tobosi District</rdfs:label>
    </owl:NamedIndividual>
    


    <!-- http://purl.obolibrary.org/obo/GAZ_00119021 -->

    <owl:NamedIndividual rdf:about="http://purl.obolibrary.org/obo/GAZ_00119021">
        <rdf:type rdf:resource="http://purl.obolibrary.org/obo/ENVO_00000004"/>
        <obo:RO_0001025 rdf:resource="http://purl.obolibrary.org/obo/GAZ_00068664"/>
        <obo:IAO_0000115>A district of El Guarco Canton.</obo:IAO_0000115>
        <oboInOwl:hasOBONamespace>GAZ</oboInOwl:hasOBONamespace>
        <oboInOwl:id>GAZ:00119021</oboInOwl:id>
        <rdfs:label>El Tejar District</rdfs:label>
    </owl:NamedIndividual>
    


    <!-- http://purl.obolibrary.org/obo/GAZ_00119022 -->

    <owl:NamedIndividual rdf:about="http://purl.obolibrary.org/obo/GAZ_00119022">
        <rdf:type rdf:resource="http://purl.obolibrary.org/obo/ENVO_00000004"/>
        <obo:RO_0001025 rdf:resource="http://purl.obolibrary.org/obo/GAZ_00068664"/>
        <obo:IAO_0000115>A district of El Guarco Canton.</obo:IAO_0000115>
        <oboInOwl:hasOBONamespace>GAZ</oboInOwl:hasOBONamespace>
        <oboInOwl:id>GAZ:00119022</oboInOwl:id>
        <rdfs:label>Patio de Agua District</rdfs:label>
    </owl:NamedIndividual>
    


    <!-- http://purl.obolibrary.org/obo/GAZ_00119023 -->

    <owl:NamedIndividual rdf:about="http://purl.obolibrary.org/obo/GAZ_00119023">
        <rdf:type rdf:resource="http://purl.obolibrary.org/obo/ENVO_00000004"/>
        <obo:RO_0001025 rdf:resource="http://purl.obolibrary.org/obo/GAZ_00068660"/>
        <obo:IAO_0000115>A district of Abangares Canton.</obo:IAO_0000115>
        <oboInOwl:hasOBONamespace>GAZ</oboInOwl:hasOBONamespace>
        <oboInOwl:id>GAZ:00119023</oboInOwl:id>
        <rdfs:label>San Juan District</rdfs:label>
    </owl:NamedIndividual>
    


    <!-- http://purl.obolibrary.org/obo/GAZ_00119024 -->

    <owl:NamedIndividual rdf:about="http://purl.obolibrary.org/obo/GAZ_00119024">
        <rdf:type rdf:resource="http://purl.obolibrary.org/obo/ENVO_00000004"/>
        <obo:RO_0001025 rdf:resource="http://purl.obolibrary.org/obo/GAZ_00068660"/>
        <obo:IAO_0000115>A district of Abangares Canton.</obo:IAO_0000115>
        <oboInOwl:hasOBONamespace>GAZ</oboInOwl:hasOBONamespace>
        <oboInOwl:id>GAZ:00119024</oboInOwl:id>
        <rdfs:label>Colorado District</rdfs:label>
    </owl:NamedIndividual>
    


    <!-- http://purl.obolibrary.org/obo/GAZ_00119025 -->

    <owl:NamedIndividual rdf:about="http://purl.obolibrary.org/obo/GAZ_00119025">
        <rdf:type rdf:resource="http://purl.obolibrary.org/obo/ENVO_00000004"/>
        <obo:RO_0001025 rdf:resource="http://purl.obolibrary.org/obo/GAZ_00068660"/>
        <obo:IAO_0000115>A district of Abangares Canton.</obo:IAO_0000115>
        <oboInOwl:hasOBONamespace>GAZ</oboInOwl:hasOBONamespace>
        <oboInOwl:id>GAZ:00119025</oboInOwl:id>
        <rdfs:label>Las Juntas District</rdfs:label>
    </owl:NamedIndividual>
    


    <!-- http://purl.obolibrary.org/obo/GAZ_00119026 -->

    <owl:NamedIndividual rdf:about="http://purl.obolibrary.org/obo/GAZ_00119026">
        <rdf:type rdf:resource="http://purl.obolibrary.org/obo/ENVO_00000004"/>
        <obo:RO_0001025 rdf:resource="http://purl.obolibrary.org/obo/GAZ_00068660"/>
        <obo:IAO_0000115>A district of Abangares Canton.</obo:IAO_0000115>
        <oboInOwl:hasOBONamespace>GAZ</oboInOwl:hasOBONamespace>
        <oboInOwl:id>GAZ:00119026</oboInOwl:id>
        <rdfs:label>La Sierra District</rdfs:label>
    </owl:NamedIndividual>
    


    <!-- http://purl.obolibrary.org/obo/GAZ_00119027 -->

    <owl:NamedIndividual rdf:about="http://purl.obolibrary.org/obo/GAZ_00119027">
        <rdf:type rdf:resource="http://purl.obolibrary.org/obo/ENVO_00000004"/>
        <obo:RO_0001025 rdf:resource="http://purl.obolibrary.org/obo/GAZ_00068675"/>
        <obo:IAO_0000115>A district of Bagaces Canton.</obo:IAO_0000115>
        <oboInOwl:hasOBONamespace>GAZ</oboInOwl:hasOBONamespace>
        <oboInOwl:id>GAZ:00119027</oboInOwl:id>
        <rdfs:label>La Fortuna District</rdfs:label>
    </owl:NamedIndividual>
    


    <!-- http://purl.obolibrary.org/obo/GAZ_00119028 -->

    <owl:NamedIndividual rdf:about="http://purl.obolibrary.org/obo/GAZ_00119028">
        <rdf:type rdf:resource="http://purl.obolibrary.org/obo/ENVO_00000004"/>
        <obo:RO_0001025 rdf:resource="http://purl.obolibrary.org/obo/GAZ_00068675"/>
        <obo:IAO_0000115>A district of Bagaces Canton.</obo:IAO_0000115>
        <oboInOwl:hasOBONamespace>GAZ</oboInOwl:hasOBONamespace>
        <oboInOwl:id>GAZ:00119028</oboInOwl:id>
        <rdfs:label>Bagaces District</rdfs:label>
    </owl:NamedIndividual>
    


    <!-- http://purl.obolibrary.org/obo/GAZ_00119029 -->

    <owl:NamedIndividual rdf:about="http://purl.obolibrary.org/obo/GAZ_00119029">
        <rdf:type rdf:resource="http://purl.obolibrary.org/obo/ENVO_00000004"/>
        <obo:RO_0001025 rdf:resource="http://purl.obolibrary.org/obo/GAZ_00068675"/>
        <obo:IAO_0000115>A district of Bagaces Canton.</obo:IAO_0000115>
        <oboInOwl:hasOBONamespace>GAZ</oboInOwl:hasOBONamespace>
        <oboInOwl:id>GAZ:00119029</oboInOwl:id>
        <rdfs:label>Rio Naranjo District</rdfs:label>
    </owl:NamedIndividual>
    


    <!-- http://purl.obolibrary.org/obo/GAZ_00119030 -->

    <owl:NamedIndividual rdf:about="http://purl.obolibrary.org/obo/GAZ_00119030">
        <rdf:type rdf:resource="http://purl.obolibrary.org/obo/ENVO_00000004"/>
        <obo:RO_0001025 rdf:resource="http://purl.obolibrary.org/obo/GAZ_00068675"/>
        <obo:IAO_0000115>A district of Bagaces Canton.</obo:IAO_0000115>
        <oboInOwl:hasOBONamespace>GAZ</oboInOwl:hasOBONamespace>
        <oboInOwl:id>GAZ:00119030</oboInOwl:id>
        <rdfs:label>Mogote District</rdfs:label>
    </owl:NamedIndividual>
    


    <!-- http://purl.obolibrary.org/obo/GAZ_00119031 -->

    <owl:NamedIndividual rdf:about="http://purl.obolibrary.org/obo/GAZ_00119031">
        <rdf:type rdf:resource="http://purl.obolibrary.org/obo/ENVO_00000004"/>
        <obo:RO_0001025 rdf:resource="http://purl.obolibrary.org/obo/GAZ_00068673"/>
        <obo:IAO_0000115>A district of Canas Canton.</obo:IAO_0000115>
        <oboInOwl:hasOBONamespace>GAZ</oboInOwl:hasOBONamespace>
        <oboInOwl:id>GAZ:00119031</oboInOwl:id>
        <rdfs:label>Porozal District</rdfs:label>
    </owl:NamedIndividual>
    


    <!-- http://purl.obolibrary.org/obo/GAZ_00119032 -->

    <owl:NamedIndividual rdf:about="http://purl.obolibrary.org/obo/GAZ_00119032">
        <rdf:type rdf:resource="http://purl.obolibrary.org/obo/ENVO_00000004"/>
        <obo:RO_0001025 rdf:resource="http://purl.obolibrary.org/obo/GAZ_00068673"/>
        <obo:IAO_0000115>A district of Canas Canton.</obo:IAO_0000115>
        <oboInOwl:hasOBONamespace>GAZ</oboInOwl:hasOBONamespace>
        <oboInOwl:id>GAZ:00119032</oboInOwl:id>
        <rdfs:label>Palmira District</rdfs:label>
    </owl:NamedIndividual>
    


    <!-- http://purl.obolibrary.org/obo/GAZ_00119033 -->

    <owl:NamedIndividual rdf:about="http://purl.obolibrary.org/obo/GAZ_00119033">
        <rdf:type rdf:resource="http://purl.obolibrary.org/obo/ENVO_00000004"/>
        <obo:RO_0001025 rdf:resource="http://purl.obolibrary.org/obo/GAZ_00068673"/>
        <obo:IAO_0000115>A district of Canas Canton.</obo:IAO_0000115>
        <oboInOwl:hasOBONamespace>GAZ</oboInOwl:hasOBONamespace>
        <oboInOwl:id>GAZ:00119033</oboInOwl:id>
        <rdfs:label>San Miguel District</rdfs:label>
    </owl:NamedIndividual>
    


    <!-- http://purl.obolibrary.org/obo/GAZ_00119034 -->

    <owl:NamedIndividual rdf:about="http://purl.obolibrary.org/obo/GAZ_00119034">
        <rdf:type rdf:resource="http://purl.obolibrary.org/obo/ENVO_00000004"/>
        <obo:RO_0001025 rdf:resource="http://purl.obolibrary.org/obo/GAZ_00068673"/>
        <obo:IAO_0000115>A district of Canas Canton.</obo:IAO_0000115>
        <oboInOwl:hasOBONamespace>GAZ</oboInOwl:hasOBONamespace>
        <oboInOwl:id>GAZ:00119034</oboInOwl:id>
        <rdfs:label>Canas District</rdfs:label>
    </owl:NamedIndividual>
    


    <!-- http://purl.obolibrary.org/obo/GAZ_00119035 -->

    <owl:NamedIndividual rdf:about="http://purl.obolibrary.org/obo/GAZ_00119035">
        <rdf:type rdf:resource="http://purl.obolibrary.org/obo/ENVO_00000004"/>
        <obo:RO_0001025 rdf:resource="http://purl.obolibrary.org/obo/GAZ_00068673"/>
        <obo:IAO_0000115>A district of Canas Canton.</obo:IAO_0000115>
        <oboInOwl:hasOBONamespace>GAZ</oboInOwl:hasOBONamespace>
        <oboInOwl:id>GAZ:00119035</oboInOwl:id>
        <rdfs:label>Bebedero District</rdfs:label>
    </owl:NamedIndividual>
    


    <!-- http://purl.obolibrary.org/obo/GAZ_00119036 -->

    <owl:NamedIndividual rdf:about="http://purl.obolibrary.org/obo/GAZ_00119036">
        <rdf:type rdf:resource="http://purl.obolibrary.org/obo/ENVO_00000004"/>
        <obo:RO_0001025 rdf:resource="http://purl.obolibrary.org/obo/GAZ_00068671"/>
        <obo:IAO_0000115>A district of Carrillo Canton.</obo:IAO_0000115>
        <oboInOwl:hasOBONamespace>GAZ</oboInOwl:hasOBONamespace>
        <oboInOwl:id>GAZ:00119036</oboInOwl:id>
        <rdfs:label>Filadelfia District</rdfs:label>
    </owl:NamedIndividual>
    


    <!-- http://purl.obolibrary.org/obo/GAZ_00119037 -->

    <owl:NamedIndividual rdf:about="http://purl.obolibrary.org/obo/GAZ_00119037">
        <rdf:type rdf:resource="http://purl.obolibrary.org/obo/ENVO_00000004"/>
        <obo:RO_0001025 rdf:resource="http://purl.obolibrary.org/obo/GAZ_00068671"/>
        <obo:IAO_0000115>A district of Carrillo Canton.</obo:IAO_0000115>
        <oboInOwl:hasOBONamespace>GAZ</oboInOwl:hasOBONamespace>
        <oboInOwl:id>GAZ:00119037</oboInOwl:id>
        <rdfs:label>Sardinal District</rdfs:label>
    </owl:NamedIndividual>
    


    <!-- http://purl.obolibrary.org/obo/GAZ_00119038 -->

    <owl:NamedIndividual rdf:about="http://purl.obolibrary.org/obo/GAZ_00119038">
        <rdf:type rdf:resource="http://purl.obolibrary.org/obo/ENVO_00000004"/>
        <obo:RO_0001025 rdf:resource="http://purl.obolibrary.org/obo/GAZ_00068671"/>
        <obo:IAO_0000115>A district of Carrillo Canton.</obo:IAO_0000115>
        <oboInOwl:hasOBONamespace>GAZ</oboInOwl:hasOBONamespace>
        <oboInOwl:id>GAZ:00119038</oboInOwl:id>
        <rdfs:label>Belen District</rdfs:label>
    </owl:NamedIndividual>
    


    <!-- http://purl.obolibrary.org/obo/GAZ_00119039 -->

    <owl:NamedIndividual rdf:about="http://purl.obolibrary.org/obo/GAZ_00119039">
        <rdf:type rdf:resource="http://purl.obolibrary.org/obo/ENVO_00000004"/>
        <obo:RO_0001025 rdf:resource="http://purl.obolibrary.org/obo/GAZ_00068671"/>
        <obo:IAO_0000115>A district of Carrillo Canton.</obo:IAO_0000115>
        <oboInOwl:hasOBONamespace>GAZ</oboInOwl:hasOBONamespace>
        <oboInOwl:id>GAZ:00119039</oboInOwl:id>
        <rdfs:label>Palmira District</rdfs:label>
    </owl:NamedIndividual>
    


    <!-- http://purl.obolibrary.org/obo/GAZ_00119040 -->

    <owl:NamedIndividual rdf:about="http://purl.obolibrary.org/obo/GAZ_00119040">
        <rdf:type rdf:resource="http://purl.obolibrary.org/obo/ENVO_00000004"/>
        <obo:RO_0001025 rdf:resource="http://purl.obolibrary.org/obo/GAZ_00068676"/>
        <obo:IAO_0000115>A district of Hojancha Canton.</obo:IAO_0000115>
        <oboInOwl:hasOBONamespace>GAZ</oboInOwl:hasOBONamespace>
        <oboInOwl:id>GAZ:00119040</oboInOwl:id>
        <rdfs:label>Huacas District</rdfs:label>
    </owl:NamedIndividual>
    


    <!-- http://purl.obolibrary.org/obo/GAZ_00119041 -->

    <owl:NamedIndividual rdf:about="http://purl.obolibrary.org/obo/GAZ_00119041">
        <rdf:type rdf:resource="http://purl.obolibrary.org/obo/ENVO_00000004"/>
        <obo:RO_0001025 rdf:resource="http://purl.obolibrary.org/obo/GAZ_00068676"/>
        <obo:IAO_0000115>A district of Hojancha Canton.</obo:IAO_0000115>
        <oboInOwl:hasOBONamespace>GAZ</oboInOwl:hasOBONamespace>
        <oboInOwl:id>GAZ:00119041</oboInOwl:id>
        <rdfs:label>Hojancha District</rdfs:label>
    </owl:NamedIndividual>
    


    <!-- http://purl.obolibrary.org/obo/GAZ_00119042 -->

    <owl:NamedIndividual rdf:about="http://purl.obolibrary.org/obo/GAZ_00119042">
        <rdf:type rdf:resource="http://purl.obolibrary.org/obo/ENVO_00000004"/>
        <obo:RO_0001025 rdf:resource="http://purl.obolibrary.org/obo/GAZ_00068676"/>
        <obo:IAO_0000115>A district of Hojancha Canton.</obo:IAO_0000115>
        <oboInOwl:hasOBONamespace>GAZ</oboInOwl:hasOBONamespace>
        <oboInOwl:id>GAZ:00119042</oboInOwl:id>
        <rdfs:label>Monte Romo District</rdfs:label>
    </owl:NamedIndividual>
    


    <!-- http://purl.obolibrary.org/obo/GAZ_00119043 -->

    <owl:NamedIndividual rdf:about="http://purl.obolibrary.org/obo/GAZ_00119043">
        <rdf:type rdf:resource="http://purl.obolibrary.org/obo/ENVO_00000004"/>
        <obo:RO_0001025 rdf:resource="http://purl.obolibrary.org/obo/GAZ_00068676"/>
        <obo:IAO_0000115>A district of Hojancha Canton.</obo:IAO_0000115>
        <oboInOwl:hasOBONamespace>GAZ</oboInOwl:hasOBONamespace>
        <oboInOwl:id>GAZ:00119043</oboInOwl:id>
        <rdfs:label>Puerto Carrillo District</rdfs:label>
    </owl:NamedIndividual>
    


    <!-- http://purl.obolibrary.org/obo/GAZ_00119044 -->

    <owl:NamedIndividual rdf:about="http://purl.obolibrary.org/obo/GAZ_00119044">
        <rdf:type rdf:resource="http://purl.obolibrary.org/obo/ENVO_00000004"/>
        <obo:RO_0001025 rdf:resource="http://purl.obolibrary.org/obo/GAZ_00068670"/>
        <obo:IAO_0000115>A district of La Cruz Canton.</obo:IAO_0000115>
        <oboInOwl:hasOBONamespace>GAZ</oboInOwl:hasOBONamespace>
        <oboInOwl:id>GAZ:00119044</oboInOwl:id>
        <rdfs:label>Santa Cecilia District</rdfs:label>
    </owl:NamedIndividual>
    


    <!-- http://purl.obolibrary.org/obo/GAZ_00119045 -->

    <owl:NamedIndividual rdf:about="http://purl.obolibrary.org/obo/GAZ_00119045">
        <rdf:type rdf:resource="http://purl.obolibrary.org/obo/ENVO_00000004"/>
        <obo:RO_0001025 rdf:resource="http://purl.obolibrary.org/obo/GAZ_00068670"/>
        <obo:IAO_0000115>A district of La Cruz Canton.</obo:IAO_0000115>
        <oboInOwl:hasOBONamespace>GAZ</oboInOwl:hasOBONamespace>
        <oboInOwl:id>GAZ:00119045</oboInOwl:id>
        <rdfs:label>La Cruz District</rdfs:label>
    </owl:NamedIndividual>
    


    <!-- http://purl.obolibrary.org/obo/GAZ_00119046 -->

    <owl:NamedIndividual rdf:about="http://purl.obolibrary.org/obo/GAZ_00119046">
        <rdf:type rdf:resource="http://purl.obolibrary.org/obo/ENVO_00000004"/>
        <obo:RO_0001025 rdf:resource="http://purl.obolibrary.org/obo/GAZ_00068670"/>
        <obo:IAO_0000115>A district of La Cruz Canton.</obo:IAO_0000115>
        <oboInOwl:hasOBONamespace>GAZ</oboInOwl:hasOBONamespace>
        <oboInOwl:id>GAZ:00119046</oboInOwl:id>
        <rdfs:label>Santa Elena District</rdfs:label>
    </owl:NamedIndividual>
    


    <!-- http://purl.obolibrary.org/obo/GAZ_00119047 -->

    <owl:NamedIndividual rdf:about="http://purl.obolibrary.org/obo/GAZ_00119047">
        <rdf:type rdf:resource="http://purl.obolibrary.org/obo/ENVO_00000004"/>
        <obo:RO_0001025 rdf:resource="http://purl.obolibrary.org/obo/GAZ_00068670"/>
        <obo:IAO_0000115>A district of La Cruz Canton.</obo:IAO_0000115>
        <oboInOwl:hasOBONamespace>GAZ</oboInOwl:hasOBONamespace>
        <oboInOwl:id>GAZ:00119047</oboInOwl:id>
        <rdfs:label>La Garita District</rdfs:label>
    </owl:NamedIndividual>
    


    <!-- http://purl.obolibrary.org/obo/GAZ_00119048 -->

    <owl:NamedIndividual rdf:about="http://purl.obolibrary.org/obo/GAZ_00119048">
        <rdf:type rdf:resource="http://purl.obolibrary.org/obo/ENVO_00000004"/>
        <obo:RO_0001025 rdf:resource="http://purl.obolibrary.org/obo/GAZ_00068677"/>
        <obo:IAO_0000115>A district of Liberia Canton.</obo:IAO_0000115>
        <oboInOwl:hasOBONamespace>GAZ</oboInOwl:hasOBONamespace>
        <oboInOwl:id>GAZ:00119048</oboInOwl:id>
        <rdfs:label>Canas Dulces District</rdfs:label>
    </owl:NamedIndividual>
    


    <!-- http://purl.obolibrary.org/obo/GAZ_00119049 -->

    <owl:NamedIndividual rdf:about="http://purl.obolibrary.org/obo/GAZ_00119049">
        <rdf:type rdf:resource="http://purl.obolibrary.org/obo/ENVO_00000004"/>
        <obo:RO_0001025 rdf:resource="http://purl.obolibrary.org/obo/GAZ_00068677"/>
        <obo:IAO_0000115>A district of Liberia Canton.</obo:IAO_0000115>
        <oboInOwl:hasOBONamespace>GAZ</oboInOwl:hasOBONamespace>
        <oboInOwl:id>GAZ:00119049</oboInOwl:id>
        <rdfs:label>Curubande District</rdfs:label>
    </owl:NamedIndividual>
    


    <!-- http://purl.obolibrary.org/obo/GAZ_00119050 -->

    <owl:NamedIndividual rdf:about="http://purl.obolibrary.org/obo/GAZ_00119050">
        <rdf:type rdf:resource="http://purl.obolibrary.org/obo/ENVO_00000004"/>
        <obo:RO_0001025 rdf:resource="http://purl.obolibrary.org/obo/GAZ_00068677"/>
        <obo:IAO_0000115>A district of Liberia Canton.</obo:IAO_0000115>
        <oboInOwl:hasOBONamespace>GAZ</oboInOwl:hasOBONamespace>
        <oboInOwl:id>GAZ:00119050</oboInOwl:id>
        <rdfs:label>Nacascolo District</rdfs:label>
    </owl:NamedIndividual>
    


    <!-- http://purl.obolibrary.org/obo/GAZ_00119051 -->

    <owl:NamedIndividual rdf:about="http://purl.obolibrary.org/obo/GAZ_00119051">
        <rdf:type rdf:resource="http://purl.obolibrary.org/obo/ENVO_00000004"/>
        <obo:RO_0001025 rdf:resource="http://purl.obolibrary.org/obo/GAZ_00068677"/>
        <obo:IAO_0000115>A district of Liberia Canton.</obo:IAO_0000115>
        <oboInOwl:hasOBONamespace>GAZ</oboInOwl:hasOBONamespace>
        <oboInOwl:id>GAZ:00119051</oboInOwl:id>
        <rdfs:label>Liberia District</rdfs:label>
    </owl:NamedIndividual>
    


    <!-- http://purl.obolibrary.org/obo/GAZ_00119052 -->

    <owl:NamedIndividual rdf:about="http://purl.obolibrary.org/obo/GAZ_00119052">
        <rdf:type rdf:resource="http://purl.obolibrary.org/obo/ENVO_00000004"/>
        <obo:RO_0001025 rdf:resource="http://purl.obolibrary.org/obo/GAZ_00068677"/>
        <obo:IAO_0000115>A district of Liberia Canton.</obo:IAO_0000115>
        <oboInOwl:hasOBONamespace>GAZ</oboInOwl:hasOBONamespace>
        <oboInOwl:id>GAZ:00119052</oboInOwl:id>
        <rdfs:label>Mayorga District</rdfs:label>
    </owl:NamedIndividual>
    


    <!-- http://purl.obolibrary.org/obo/GAZ_00119053 -->

    <owl:NamedIndividual rdf:about="http://purl.obolibrary.org/obo/GAZ_00119053">
        <rdf:type rdf:resource="http://purl.obolibrary.org/obo/ENVO_00000004"/>
        <obo:RO_0001025 rdf:resource="http://purl.obolibrary.org/obo/GAZ_00068669"/>
        <obo:IAO_0000115>A district of Nandayure Canton.</obo:IAO_0000115>
        <oboInOwl:hasOBONamespace>GAZ</oboInOwl:hasOBONamespace>
        <oboInOwl:id>GAZ:00119053</oboInOwl:id>
        <rdfs:label>Carmona District</rdfs:label>
    </owl:NamedIndividual>
    


    <!-- http://purl.obolibrary.org/obo/GAZ_00119054 -->

    <owl:NamedIndividual rdf:about="http://purl.obolibrary.org/obo/GAZ_00119054">
        <rdf:type rdf:resource="http://purl.obolibrary.org/obo/ENVO_00000004"/>
        <obo:RO_0001025 rdf:resource="http://purl.obolibrary.org/obo/GAZ_00068669"/>
        <obo:IAO_0000115>A district of Nandayure Canton.</obo:IAO_0000115>
        <oboInOwl:hasOBONamespace>GAZ</oboInOwl:hasOBONamespace>
        <oboInOwl:id>GAZ:00119054</oboInOwl:id>
        <rdfs:label>Santa Rita District</rdfs:label>
    </owl:NamedIndividual>
    


    <!-- http://purl.obolibrary.org/obo/GAZ_00119055 -->

    <owl:NamedIndividual rdf:about="http://purl.obolibrary.org/obo/GAZ_00119055">
        <rdf:type rdf:resource="http://purl.obolibrary.org/obo/ENVO_00000004"/>
        <obo:RO_0001025 rdf:resource="http://purl.obolibrary.org/obo/GAZ_00068669"/>
        <obo:IAO_0000115>A district of Nandayure Canton.</obo:IAO_0000115>
        <oboInOwl:hasOBONamespace>GAZ</oboInOwl:hasOBONamespace>
        <oboInOwl:id>GAZ:00119055</oboInOwl:id>
        <rdfs:label>Zapotal District</rdfs:label>
    </owl:NamedIndividual>
    


    <!-- http://purl.obolibrary.org/obo/GAZ_00119056 -->

    <owl:NamedIndividual rdf:about="http://purl.obolibrary.org/obo/GAZ_00119056">
        <rdf:type rdf:resource="http://purl.obolibrary.org/obo/ENVO_00000004"/>
        <obo:RO_0001025 rdf:resource="http://purl.obolibrary.org/obo/GAZ_00068669"/>
        <obo:IAO_0000115>A district of Nandayure Canton.</obo:IAO_0000115>
        <oboInOwl:hasOBONamespace>GAZ</oboInOwl:hasOBONamespace>
        <oboInOwl:id>GAZ:00119056</oboInOwl:id>
        <rdfs:label>Bejuco District</rdfs:label>
    </owl:NamedIndividual>
    


    <!-- http://purl.obolibrary.org/obo/GAZ_00119057 -->

    <owl:NamedIndividual rdf:about="http://purl.obolibrary.org/obo/GAZ_00119057">
        <rdf:type rdf:resource="http://purl.obolibrary.org/obo/ENVO_00000004"/>
        <obo:RO_0001025 rdf:resource="http://purl.obolibrary.org/obo/GAZ_00068669"/>
        <obo:IAO_0000115>A district of Nandayure Canton.</obo:IAO_0000115>
        <oboInOwl:hasOBONamespace>GAZ</oboInOwl:hasOBONamespace>
        <oboInOwl:id>GAZ:00119057</oboInOwl:id>
        <rdfs:label>San Pablo District</rdfs:label>
    </owl:NamedIndividual>
    


    <!-- http://purl.obolibrary.org/obo/GAZ_00119058 -->

    <owl:NamedIndividual rdf:about="http://purl.obolibrary.org/obo/GAZ_00119058">
        <rdf:type rdf:resource="http://purl.obolibrary.org/obo/ENVO_00000004"/>
        <obo:RO_0001025 rdf:resource="http://purl.obolibrary.org/obo/GAZ_00068669"/>
        <obo:IAO_0000115>A district of Nandayure Canton.</obo:IAO_0000115>
        <oboInOwl:hasOBONamespace>GAZ</oboInOwl:hasOBONamespace>
        <oboInOwl:id>GAZ:00119058</oboInOwl:id>
        <rdfs:label>Porvenir District</rdfs:label>
    </owl:NamedIndividual>
    


    <!-- http://purl.obolibrary.org/obo/GAZ_00119059 -->

    <owl:NamedIndividual rdf:about="http://purl.obolibrary.org/obo/GAZ_00119059">
        <rdf:type rdf:resource="http://purl.obolibrary.org/obo/ENVO_00000004"/>
        <obo:RO_0001025 rdf:resource="http://purl.obolibrary.org/obo/GAZ_00068678"/>
        <obo:IAO_0000115>A district of Nicoya Canton.</obo:IAO_0000115>
        <oboInOwl:hasOBONamespace>GAZ</oboInOwl:hasOBONamespace>
        <oboInOwl:id>GAZ:00119059</oboInOwl:id>
        <rdfs:label>Mansion District</rdfs:label>
    </owl:NamedIndividual>
    


    <!-- http://purl.obolibrary.org/obo/GAZ_00119060 -->

    <owl:NamedIndividual rdf:about="http://purl.obolibrary.org/obo/GAZ_00119060">
        <rdf:type rdf:resource="http://purl.obolibrary.org/obo/ENVO_00000004"/>
        <obo:RO_0001025 rdf:resource="http://purl.obolibrary.org/obo/GAZ_00068678"/>
        <obo:IAO_0000115>A district of Nicoya Canton.</obo:IAO_0000115>
        <oboInOwl:hasOBONamespace>GAZ</oboInOwl:hasOBONamespace>
        <oboInOwl:id>GAZ:00119060</oboInOwl:id>
        <rdfs:label>Quebrada Honda District</rdfs:label>
    </owl:NamedIndividual>
    


    <!-- http://purl.obolibrary.org/obo/GAZ_00119061 -->

    <owl:NamedIndividual rdf:about="http://purl.obolibrary.org/obo/GAZ_00119061">
        <rdf:type rdf:resource="http://purl.obolibrary.org/obo/ENVO_00000004"/>
        <obo:RO_0001025 rdf:resource="http://purl.obolibrary.org/obo/GAZ_00068678"/>
        <obo:IAO_0000115>A district of Nicoya Canton.</obo:IAO_0000115>
        <oboInOwl:hasOBONamespace>GAZ</oboInOwl:hasOBONamespace>
        <oboInOwl:id>GAZ:00119061</oboInOwl:id>
        <rdfs:label>Nicoya District</rdfs:label>
    </owl:NamedIndividual>
    


    <!-- http://purl.obolibrary.org/obo/GAZ_00119062 -->

    <owl:NamedIndividual rdf:about="http://purl.obolibrary.org/obo/GAZ_00119062">
        <rdf:type rdf:resource="http://purl.obolibrary.org/obo/ENVO_00000004"/>
        <obo:RO_0001025 rdf:resource="http://purl.obolibrary.org/obo/GAZ_00068678"/>
        <obo:IAO_0000115>A district of Nicoya Canton.</obo:IAO_0000115>
        <oboInOwl:hasOBONamespace>GAZ</oboInOwl:hasOBONamespace>
        <oboInOwl:id>GAZ:00119062</oboInOwl:id>
        <rdfs:label>San Antonio District</rdfs:label>
    </owl:NamedIndividual>
    


    <!-- http://purl.obolibrary.org/obo/GAZ_00119063 -->

    <owl:NamedIndividual rdf:about="http://purl.obolibrary.org/obo/GAZ_00119063">
        <rdf:type rdf:resource="http://purl.obolibrary.org/obo/ENVO_00000004"/>
        <obo:RO_0001025 rdf:resource="http://purl.obolibrary.org/obo/GAZ_00068678"/>
        <obo:IAO_0000115>A district of Nicoya Canton.</obo:IAO_0000115>
        <oboInOwl:hasOBONamespace>GAZ</oboInOwl:hasOBONamespace>
        <oboInOwl:id>GAZ:00119063</oboInOwl:id>
        <rdfs:label>Nosara District</rdfs:label>
    </owl:NamedIndividual>
    


    <!-- http://purl.obolibrary.org/obo/GAZ_00119064 -->

    <owl:NamedIndividual rdf:about="http://purl.obolibrary.org/obo/GAZ_00119064">
        <rdf:type rdf:resource="http://purl.obolibrary.org/obo/ENVO_00000004"/>
        <obo:RO_0001025 rdf:resource="http://purl.obolibrary.org/obo/GAZ_00068678"/>
        <obo:IAO_0000115>A district of Nicoya Canton.</obo:IAO_0000115>
        <oboInOwl:hasOBONamespace>GAZ</oboInOwl:hasOBONamespace>
        <oboInOwl:id>GAZ:00119064</oboInOwl:id>
        <rdfs:label>Samara District</rdfs:label>
    </owl:NamedIndividual>
    


    <!-- http://purl.obolibrary.org/obo/GAZ_00119065 -->

    <owl:NamedIndividual rdf:about="http://purl.obolibrary.org/obo/GAZ_00119065">
        <rdf:type rdf:resource="http://purl.obolibrary.org/obo/ENVO_00000004"/>
        <obo:RO_0001025 rdf:resource="http://purl.obolibrary.org/obo/GAZ_00068678"/>
        <obo:IAO_0000115>A district of Nicoya Canton.</obo:IAO_0000115>
        <oboInOwl:hasOBONamespace>GAZ</oboInOwl:hasOBONamespace>
        <oboInOwl:id>GAZ:00119065</oboInOwl:id>
        <rdfs:label>Belen de Nosarita District</rdfs:label>
    </owl:NamedIndividual>
    


    <!-- http://purl.obolibrary.org/obo/GAZ_00119066 -->

    <owl:NamedIndividual rdf:about="http://purl.obolibrary.org/obo/GAZ_00119066">
        <obo:RO_0001025 rdf:resource="http://purl.obolibrary.org/obo/GAZ_00068872"/>
        <oboInOwl:hasOBONamespace>GAZ</oboInOwl:hasOBONamespace>
        <oboInOwl:id>GAZ:00119066</oboInOwl:id>
        <rdfs:label>Laguna del Paraguas</rdfs:label>
    </owl:NamedIndividual>
    


    <!-- http://purl.obolibrary.org/obo/GAZ_00119067 -->

    <owl:NamedIndividual rdf:about="http://purl.obolibrary.org/obo/GAZ_00119067">
        <rdf:type rdf:resource="http://purl.obolibrary.org/obo/ENVO_00000004"/>
        <obo:RO_0001025 rdf:resource="http://purl.obolibrary.org/obo/GAZ_00068672"/>
        <obo:IAO_0000115>A district of Santa Cruz Canton.</obo:IAO_0000115>
        <oboInOwl:hasOBONamespace>GAZ</oboInOwl:hasOBONamespace>
        <oboInOwl:id>GAZ:00119067</oboInOwl:id>
        <rdfs:label>Santa Cruz District</rdfs:label>
    </owl:NamedIndividual>
    


    <!-- http://purl.obolibrary.org/obo/GAZ_00119068 -->

    <owl:NamedIndividual rdf:about="http://purl.obolibrary.org/obo/GAZ_00119068">
        <rdf:type rdf:resource="http://purl.obolibrary.org/obo/ENVO_00000004"/>
        <obo:RO_0001025 rdf:resource="http://purl.obolibrary.org/obo/GAZ_00068672"/>
        <obo:IAO_0000115>A district of Santa Cruz Canton.</obo:IAO_0000115>
        <oboInOwl:hasOBONamespace>GAZ</oboInOwl:hasOBONamespace>
        <oboInOwl:id>GAZ:00119068</oboInOwl:id>
        <rdfs:label>Cuajiniquil District</rdfs:label>
    </owl:NamedIndividual>
    


    <!-- http://purl.obolibrary.org/obo/GAZ_00119069 -->

    <owl:NamedIndividual rdf:about="http://purl.obolibrary.org/obo/GAZ_00119069">
        <rdf:type rdf:resource="http://purl.obolibrary.org/obo/ENVO_00000004"/>
        <obo:RO_0001025 rdf:resource="http://purl.obolibrary.org/obo/GAZ_00068672"/>
        <obo:IAO_0000115>A district of Santa Cruz Canton.</obo:IAO_0000115>
        <oboInOwl:hasOBONamespace>GAZ</oboInOwl:hasOBONamespace>
        <oboInOwl:id>GAZ:00119069</oboInOwl:id>
        <rdfs:label>Tempate District</rdfs:label>
    </owl:NamedIndividual>
    


    <!-- http://purl.obolibrary.org/obo/GAZ_00119070 -->

    <owl:NamedIndividual rdf:about="http://purl.obolibrary.org/obo/GAZ_00119070">
        <rdf:type rdf:resource="http://purl.obolibrary.org/obo/ENVO_00000004"/>
        <obo:RO_0001025 rdf:resource="http://purl.obolibrary.org/obo/GAZ_00068672"/>
        <obo:IAO_0000115>A district of Santa Cruz Canton.</obo:IAO_0000115>
        <oboInOwl:hasOBONamespace>GAZ</oboInOwl:hasOBONamespace>
        <oboInOwl:id>GAZ:00119070</oboInOwl:id>
        <rdfs:label>Tamarindo District</rdfs:label>
    </owl:NamedIndividual>
    


    <!-- http://purl.obolibrary.org/obo/GAZ_00119071 -->

    <owl:NamedIndividual rdf:about="http://purl.obolibrary.org/obo/GAZ_00119071">
        <rdf:type rdf:resource="http://purl.obolibrary.org/obo/ENVO_00000004"/>
        <obo:RO_0001025 rdf:resource="http://purl.obolibrary.org/obo/GAZ_00068672"/>
        <obo:IAO_0000115>A district of Santa Cruz Canton.</obo:IAO_0000115>
        <oboInOwl:hasOBONamespace>GAZ</oboInOwl:hasOBONamespace>
        <oboInOwl:id>GAZ:00119071</oboInOwl:id>
        <rdfs:label>Cartagena District</rdfs:label>
    </owl:NamedIndividual>
    


    <!-- http://purl.obolibrary.org/obo/GAZ_00119072 -->

    <owl:NamedIndividual rdf:about="http://purl.obolibrary.org/obo/GAZ_00119072">
        <rdf:type rdf:resource="http://purl.obolibrary.org/obo/ENVO_00000004"/>
        <obo:RO_0001025 rdf:resource="http://purl.obolibrary.org/obo/GAZ_00068672"/>
        <obo:IAO_0000115>A district of Santa Cruz Canton.</obo:IAO_0000115>
        <oboInOwl:hasOBONamespace>GAZ</oboInOwl:hasOBONamespace>
        <oboInOwl:id>GAZ:00119072</oboInOwl:id>
        <rdfs:label>Cabo Velas District</rdfs:label>
    </owl:NamedIndividual>
    


    <!-- http://purl.obolibrary.org/obo/GAZ_00119073 -->

    <owl:NamedIndividual rdf:about="http://purl.obolibrary.org/obo/GAZ_00119073">
        <rdf:type rdf:resource="http://purl.obolibrary.org/obo/ENVO_00000004"/>
        <obo:RO_0001025 rdf:resource="http://purl.obolibrary.org/obo/GAZ_00068672"/>
        <obo:IAO_0000115>A district of Santa Cruz Canton.</obo:IAO_0000115>
        <oboInOwl:hasOBONamespace>GAZ</oboInOwl:hasOBONamespace>
        <oboInOwl:id>GAZ:00119073</oboInOwl:id>
        <rdfs:label>Veintisiete de Abril District</rdfs:label>
    </owl:NamedIndividual>
    


    <!-- http://purl.obolibrary.org/obo/GAZ_00119074 -->

    <owl:NamedIndividual rdf:about="http://purl.obolibrary.org/obo/GAZ_00119074">
        <rdf:type rdf:resource="http://purl.obolibrary.org/obo/ENVO_00000004"/>
        <obo:RO_0001025 rdf:resource="http://purl.obolibrary.org/obo/GAZ_00068672"/>
        <obo:IAO_0000115>A district of Santa Cruz Canton.</obo:IAO_0000115>
        <oboInOwl:hasOBONamespace>GAZ</oboInOwl:hasOBONamespace>
        <oboInOwl:id>GAZ:00119074</oboInOwl:id>
        <rdfs:label>Bolson District</rdfs:label>
    </owl:NamedIndividual>
    


    <!-- http://purl.obolibrary.org/obo/GAZ_00119075 -->

    <owl:NamedIndividual rdf:about="http://purl.obolibrary.org/obo/GAZ_00119075">
        <rdf:type rdf:resource="http://purl.obolibrary.org/obo/ENVO_00000004"/>
        <obo:RO_0001025 rdf:resource="http://purl.obolibrary.org/obo/GAZ_00068672"/>
        <obo:IAO_0000115>A district of Santa Cruz Canton.</obo:IAO_0000115>
        <oboInOwl:hasOBONamespace>GAZ</oboInOwl:hasOBONamespace>
        <oboInOwl:id>GAZ:00119075</oboInOwl:id>
        <rdfs:label>Diria District</rdfs:label>
    </owl:NamedIndividual>
    


    <!-- http://purl.obolibrary.org/obo/GAZ_00119076 -->

    <owl:NamedIndividual rdf:about="http://purl.obolibrary.org/obo/GAZ_00119076">
        <rdf:type rdf:resource="http://purl.obolibrary.org/obo/ENVO_00000004"/>
        <obo:RO_0001025 rdf:resource="http://purl.obolibrary.org/obo/GAZ_00068674"/>
        <obo:IAO_0000115>A district of Tilaran Canton.</obo:IAO_0000115>
        <oboInOwl:hasOBONamespace>GAZ</oboInOwl:hasOBONamespace>
        <oboInOwl:id>GAZ:00119076</oboInOwl:id>
        <rdfs:label>Santa Rosa District</rdfs:label>
    </owl:NamedIndividual>
    


    <!-- http://purl.obolibrary.org/obo/GAZ_00119077 -->

    <owl:NamedIndividual rdf:about="http://purl.obolibrary.org/obo/GAZ_00119077">
        <rdf:type rdf:resource="http://purl.obolibrary.org/obo/ENVO_00000004"/>
        <obo:RO_0001025 rdf:resource="http://purl.obolibrary.org/obo/GAZ_00068674"/>
        <obo:IAO_0000115>A district of Tilaran Canton.</obo:IAO_0000115>
        <oboInOwl:hasOBONamespace>GAZ</oboInOwl:hasOBONamespace>
        <oboInOwl:id>GAZ:00119077</oboInOwl:id>
        <rdfs:label>Nuevo Arenal District</rdfs:label>
    </owl:NamedIndividual>
    


    <!-- http://purl.obolibrary.org/obo/GAZ_00119078 -->

    <owl:NamedIndividual rdf:about="http://purl.obolibrary.org/obo/GAZ_00119078">
        <rdf:type rdf:resource="http://purl.obolibrary.org/obo/ENVO_00000004"/>
        <obo:RO_0001025 rdf:resource="http://purl.obolibrary.org/obo/GAZ_00068674"/>
        <obo:IAO_0000115>A district of Tilaran Canton.</obo:IAO_0000115>
        <oboInOwl:hasOBONamespace>GAZ</oboInOwl:hasOBONamespace>
        <oboInOwl:id>GAZ:00119078</oboInOwl:id>
        <rdfs:label>Tilaran District</rdfs:label>
    </owl:NamedIndividual>
    


    <!-- http://purl.obolibrary.org/obo/GAZ_00119079 -->

    <owl:NamedIndividual rdf:about="http://purl.obolibrary.org/obo/GAZ_00119079">
        <rdf:type rdf:resource="http://purl.obolibrary.org/obo/ENVO_00000004"/>
        <obo:RO_0001025 rdf:resource="http://purl.obolibrary.org/obo/GAZ_00068674"/>
        <obo:IAO_0000115>A district of Tilaran Canton.</obo:IAO_0000115>
        <oboInOwl:hasOBONamespace>GAZ</oboInOwl:hasOBONamespace>
        <oboInOwl:id>GAZ:00119079</oboInOwl:id>
        <rdfs:label>Quebrada Grande District</rdfs:label>
    </owl:NamedIndividual>
    


    <!-- http://purl.obolibrary.org/obo/GAZ_00119080 -->

    <owl:NamedIndividual rdf:about="http://purl.obolibrary.org/obo/GAZ_00119080">
        <rdf:type rdf:resource="http://purl.obolibrary.org/obo/ENVO_00000004"/>
        <obo:RO_0001025 rdf:resource="http://purl.obolibrary.org/obo/GAZ_00068674"/>
        <obo:IAO_0000115>A district of Tilaran Canton.</obo:IAO_0000115>
        <oboInOwl:hasOBONamespace>GAZ</oboInOwl:hasOBONamespace>
        <oboInOwl:id>GAZ:00119080</oboInOwl:id>
        <rdfs:label>Libano District</rdfs:label>
    </owl:NamedIndividual>
    


    <!-- http://purl.obolibrary.org/obo/GAZ_00119081 -->

    <owl:NamedIndividual rdf:about="http://purl.obolibrary.org/obo/GAZ_00119081">
        <rdf:type rdf:resource="http://purl.obolibrary.org/obo/ENVO_00000004"/>
        <obo:RO_0001025 rdf:resource="http://purl.obolibrary.org/obo/GAZ_00068674"/>
        <obo:IAO_0000115>A district of Tilaran Canton.</obo:IAO_0000115>
        <oboInOwl:hasOBONamespace>GAZ</oboInOwl:hasOBONamespace>
        <oboInOwl:id>GAZ:00119081</oboInOwl:id>
        <rdfs:label>Nuevo Tronadora District</rdfs:label>
    </owl:NamedIndividual>
    


    <!-- http://purl.obolibrary.org/obo/GAZ_00119082 -->

    <owl:NamedIndividual rdf:about="http://purl.obolibrary.org/obo/GAZ_00119082">
        <rdf:type rdf:resource="http://purl.obolibrary.org/obo/ENVO_00000004"/>
        <obo:RO_0001025 rdf:resource="http://purl.obolibrary.org/obo/GAZ_00068674"/>
        <obo:IAO_0000115>A district of Tilaran Canton.</obo:IAO_0000115>
        <oboInOwl:hasOBONamespace>GAZ</oboInOwl:hasOBONamespace>
        <oboInOwl:id>GAZ:00119082</oboInOwl:id>
        <rdfs:label>Tierras Morenas District</rdfs:label>
    </owl:NamedIndividual>
    


    <!-- http://purl.obolibrary.org/obo/GAZ_00119083 -->

    <owl:NamedIndividual rdf:about="http://purl.obolibrary.org/obo/GAZ_00119083">
        <obo:RO_0001025 rdf:resource="http://purl.obolibrary.org/obo/GAZ_00068905"/>
        <obo:IAO_0000115>A crater lake.</obo:IAO_0000115>
        <oboInOwl:hasOBONamespace>GAZ</oboInOwl:hasOBONamespace>
        <oboInOwl:id>GAZ:00119083</oboInOwl:id>
        <rdfs:label>Bosque Alegre Lake</rdfs:label>
    </owl:NamedIndividual>
    


    <!-- http://purl.obolibrary.org/obo/GAZ_00119084 -->

    <owl:NamedIndividual rdf:about="http://purl.obolibrary.org/obo/GAZ_00119084">
        <obo:RO_0001025 rdf:resource="http://purl.obolibrary.org/obo/GAZ_00068905"/>
        <obo:IAO_0000115>A crater lake.</obo:IAO_0000115>
        <oboInOwl:hasOBONamespace>GAZ</oboInOwl:hasOBONamespace>
        <oboInOwl:id>GAZ:00119084</oboInOwl:id>
        <rdfs:label>Hule Lake</rdfs:label>
    </owl:NamedIndividual>
    


    <!-- http://purl.obolibrary.org/obo/GAZ_00119085 -->

    <owl:NamedIndividual rdf:about="http://purl.obolibrary.org/obo/GAZ_00119085">
        <obo:RO_0001025 rdf:resource="http://purl.obolibrary.org/obo/GAZ_00068905"/>
        <obo:IAO_0000115>A crater lake.</obo:IAO_0000115>
        <oboInOwl:hasOBONamespace>GAZ</oboInOwl:hasOBONamespace>
        <oboInOwl:id>GAZ:00119085</oboInOwl:id>
        <rdfs:label>Congo Lake</rdfs:label>
    </owl:NamedIndividual>
    


    <!-- http://purl.obolibrary.org/obo/GAZ_00119086 -->

    <owl:NamedIndividual rdf:about="http://purl.obolibrary.org/obo/GAZ_00119086">
        <rdf:type rdf:resource="http://purl.obolibrary.org/obo/ENVO_00000004"/>
        <obo:RO_0001025 rdf:resource="http://purl.obolibrary.org/obo/GAZ_00068703"/>
        <obo:IAO_0000115>A district of Heredia Canton.</obo:IAO_0000115>
        <oboInOwl:hasOBONamespace>GAZ</oboInOwl:hasOBONamespace>
        <oboInOwl:id>GAZ:00119086</oboInOwl:id>
        <rdfs:label>Heredia District</rdfs:label>
    </owl:NamedIndividual>
    


    <!-- http://purl.obolibrary.org/obo/GAZ_00119087 -->

    <owl:NamedIndividual rdf:about="http://purl.obolibrary.org/obo/GAZ_00119087">
        <rdf:type rdf:resource="http://purl.obolibrary.org/obo/ENVO_00000004"/>
        <obo:RO_0001025 rdf:resource="http://purl.obolibrary.org/obo/GAZ_00068703"/>
        <obo:IAO_0000115>A district of Heredia Canton.</obo:IAO_0000115>
        <oboInOwl:hasOBONamespace>GAZ</oboInOwl:hasOBONamespace>
        <oboInOwl:id>GAZ:00119087</oboInOwl:id>
        <rdfs:label>Varablanca District</rdfs:label>
    </owl:NamedIndividual>
    


    <!-- http://purl.obolibrary.org/obo/GAZ_00119088 -->

    <owl:NamedIndividual rdf:about="http://purl.obolibrary.org/obo/GAZ_00119088">
        <rdf:type rdf:resource="http://purl.obolibrary.org/obo/ENVO_00000004"/>
        <obo:RO_0001025 rdf:resource="http://purl.obolibrary.org/obo/GAZ_00068703"/>
        <obo:IAO_0000115>A district of Heredia Canton.</obo:IAO_0000115>
        <oboInOwl:hasOBONamespace>GAZ</oboInOwl:hasOBONamespace>
        <oboInOwl:id>GAZ:00119088</oboInOwl:id>
        <rdfs:label>San Francisco District</rdfs:label>
    </owl:NamedIndividual>
    


    <!-- http://purl.obolibrary.org/obo/GAZ_00119089 -->

    <owl:NamedIndividual rdf:about="http://purl.obolibrary.org/obo/GAZ_00119089">
        <rdf:type rdf:resource="http://purl.obolibrary.org/obo/ENVO_00000004"/>
        <obo:RO_0001025 rdf:resource="http://purl.obolibrary.org/obo/GAZ_00068703"/>
        <obo:IAO_0000115>A district of Heredia Canton.</obo:IAO_0000115>
        <oboInOwl:hasOBONamespace>GAZ</oboInOwl:hasOBONamespace>
        <oboInOwl:id>GAZ:00119089</oboInOwl:id>
        <rdfs:label>Mercedes District</rdfs:label>
    </owl:NamedIndividual>
    


    <!-- http://purl.obolibrary.org/obo/GAZ_00119090 -->

    <owl:NamedIndividual rdf:about="http://purl.obolibrary.org/obo/GAZ_00119090">
        <rdf:type rdf:resource="http://purl.obolibrary.org/obo/ENVO_00000004"/>
        <obo:RO_0001025 rdf:resource="http://purl.obolibrary.org/obo/GAZ_00068703"/>
        <obo:IAO_0000115>A district of Heredia Canton.</obo:IAO_0000115>
        <oboInOwl:hasOBONamespace>GAZ</oboInOwl:hasOBONamespace>
        <oboInOwl:id>GAZ:00119090</oboInOwl:id>
        <rdfs:label>Ulloa District</rdfs:label>
    </owl:NamedIndividual>
    


    <!-- http://purl.obolibrary.org/obo/GAZ_00119091 -->

    <owl:NamedIndividual rdf:about="http://purl.obolibrary.org/obo/GAZ_00119091">
        <rdf:type rdf:resource="http://purl.obolibrary.org/obo/ENVO_00000004"/>
        <obo:RO_0001025 rdf:resource="http://purl.obolibrary.org/obo/GAZ_00068702"/>
        <obo:IAO_0000115>A district of Barva Canton.</obo:IAO_0000115>
        <oboInOwl:hasOBONamespace>GAZ</oboInOwl:hasOBONamespace>
        <oboInOwl:id>GAZ:00119091</oboInOwl:id>
        <rdfs:label>San Pedro District</rdfs:label>
    </owl:NamedIndividual>
    


    <!-- http://purl.obolibrary.org/obo/GAZ_00119092 -->

    <owl:NamedIndividual rdf:about="http://purl.obolibrary.org/obo/GAZ_00119092">
        <rdf:type rdf:resource="http://purl.obolibrary.org/obo/ENVO_00000004"/>
        <obo:RO_0001025 rdf:resource="http://purl.obolibrary.org/obo/GAZ_00068702"/>
        <obo:IAO_0000115>A district of Barva Canton.</obo:IAO_0000115>
        <oboInOwl:hasOBONamespace>GAZ</oboInOwl:hasOBONamespace>
        <oboInOwl:id>GAZ:00119092</oboInOwl:id>
        <rdfs:label>San Roque District</rdfs:label>
    </owl:NamedIndividual>
    


    <!-- http://purl.obolibrary.org/obo/GAZ_00119093 -->

    <owl:NamedIndividual rdf:about="http://purl.obolibrary.org/obo/GAZ_00119093">
        <rdf:type rdf:resource="http://purl.obolibrary.org/obo/ENVO_00000004"/>
        <obo:RO_0001025 rdf:resource="http://purl.obolibrary.org/obo/GAZ_00068702"/>
        <obo:IAO_0000115>A district of Barva Canton.</obo:IAO_0000115>
        <oboInOwl:hasOBONamespace>GAZ</oboInOwl:hasOBONamespace>
        <oboInOwl:id>GAZ:00119093</oboInOwl:id>
        <rdfs:label>San Jose de la Montana District</rdfs:label>
    </owl:NamedIndividual>
    


    <!-- http://purl.obolibrary.org/obo/GAZ_00119094 -->

    <owl:NamedIndividual rdf:about="http://purl.obolibrary.org/obo/GAZ_00119094">
        <rdf:type rdf:resource="http://purl.obolibrary.org/obo/ENVO_00000004"/>
        <obo:RO_0001025 rdf:resource="http://purl.obolibrary.org/obo/GAZ_00068702"/>
        <obo:IAO_0000115>A district of Barva Canton.</obo:IAO_0000115>
        <oboInOwl:hasOBONamespace>GAZ</oboInOwl:hasOBONamespace>
        <oboInOwl:id>GAZ:00119094</oboInOwl:id>
        <rdfs:label>Barva District</rdfs:label>
    </owl:NamedIndividual>
    


    <!-- http://purl.obolibrary.org/obo/GAZ_00119095 -->

    <owl:NamedIndividual rdf:about="http://purl.obolibrary.org/obo/GAZ_00119095">
        <rdf:type rdf:resource="http://purl.obolibrary.org/obo/ENVO_00000004"/>
        <obo:RO_0001025 rdf:resource="http://purl.obolibrary.org/obo/GAZ_00068702"/>
        <obo:IAO_0000115>A district of Barva Canton.</obo:IAO_0000115>
        <oboInOwl:hasOBONamespace>GAZ</oboInOwl:hasOBONamespace>
        <oboInOwl:id>GAZ:00119095</oboInOwl:id>
        <rdfs:label>San Pablo District</rdfs:label>
    </owl:NamedIndividual>
    


    <!-- http://purl.obolibrary.org/obo/GAZ_00119096 -->

    <owl:NamedIndividual rdf:about="http://purl.obolibrary.org/obo/GAZ_00119096">
        <rdf:type rdf:resource="http://purl.obolibrary.org/obo/ENVO_00000004"/>
        <obo:RO_0001025 rdf:resource="http://purl.obolibrary.org/obo/GAZ_00068702"/>
        <obo:IAO_0000115>A district of Barva Canton.</obo:IAO_0000115>
        <oboInOwl:hasOBONamespace>GAZ</oboInOwl:hasOBONamespace>
        <oboInOwl:id>GAZ:00119096</oboInOwl:id>
        <rdfs:label>Santa Lucia District</rdfs:label>
    </owl:NamedIndividual>
    


    <!-- http://purl.obolibrary.org/obo/GAZ_00119097 -->

    <owl:NamedIndividual rdf:about="http://purl.obolibrary.org/obo/GAZ_00119097">
        <rdf:type rdf:resource="http://purl.obolibrary.org/obo/ENVO_00000004"/>
        <obo:RO_0001025 rdf:resource="http://purl.obolibrary.org/obo/GAZ_00068707"/>
        <obo:IAO_0000115>A district of Santo Domingo Canton.</obo:IAO_0000115>
        <oboInOwl:hasOBONamespace>GAZ</oboInOwl:hasOBONamespace>
        <oboInOwl:id>GAZ:00119097</oboInOwl:id>
        <rdfs:label>Para District</rdfs:label>
    </owl:NamedIndividual>
    


    <!-- http://purl.obolibrary.org/obo/GAZ_00119098 -->

    <owl:NamedIndividual rdf:about="http://purl.obolibrary.org/obo/GAZ_00119098">
        <rdf:type rdf:resource="http://purl.obolibrary.org/obo/ENVO_00000004"/>
        <obo:RO_0001025 rdf:resource="http://purl.obolibrary.org/obo/GAZ_00068707"/>
        <obo:IAO_0000115>A district of Santo Domingo Canton.</obo:IAO_0000115>
        <oboInOwl:hasOBONamespace>GAZ</oboInOwl:hasOBONamespace>
        <oboInOwl:id>GAZ:00119098</oboInOwl:id>
        <rdfs:label>San Vicente District</rdfs:label>
    </owl:NamedIndividual>
    


    <!-- http://purl.obolibrary.org/obo/GAZ_00119099 -->

    <owl:NamedIndividual rdf:about="http://purl.obolibrary.org/obo/GAZ_00119099">
        <rdf:type rdf:resource="http://purl.obolibrary.org/obo/ENVO_00000004"/>
        <obo:RO_0001025 rdf:resource="http://purl.obolibrary.org/obo/GAZ_00068707"/>
        <obo:IAO_0000115>A district of Santo Domingo Canton.</obo:IAO_0000115>
        <oboInOwl:hasOBONamespace>GAZ</oboInOwl:hasOBONamespace>
        <oboInOwl:id>GAZ:00119099</oboInOwl:id>
        <rdfs:label>Santo Tomas District</rdfs:label>
    </owl:NamedIndividual>
    


    <!-- http://purl.obolibrary.org/obo/GAZ_00119100 -->

    <owl:NamedIndividual rdf:about="http://purl.obolibrary.org/obo/GAZ_00119100">
        <rdf:type rdf:resource="http://purl.obolibrary.org/obo/ENVO_00000004"/>
        <obo:RO_0001025 rdf:resource="http://purl.obolibrary.org/obo/GAZ_00068707"/>
        <obo:IAO_0000115>A district of Santo Domingo Canton.</obo:IAO_0000115>
        <oboInOwl:hasOBONamespace>GAZ</oboInOwl:hasOBONamespace>
        <oboInOwl:id>GAZ:00119100</oboInOwl:id>
        <rdfs:label>Tures District</rdfs:label>
    </owl:NamedIndividual>
    


    <!-- http://purl.obolibrary.org/obo/GAZ_00119101 -->

    <owl:NamedIndividual rdf:about="http://purl.obolibrary.org/obo/GAZ_00119101">
        <rdf:type rdf:resource="http://purl.obolibrary.org/obo/ENVO_00000004"/>
        <obo:RO_0001025 rdf:resource="http://purl.obolibrary.org/obo/GAZ_00068707"/>
        <obo:IAO_0000115>A district of Santo Domingo Canton.</obo:IAO_0000115>
        <oboInOwl:hasOBONamespace>GAZ</oboInOwl:hasOBONamespace>
        <oboInOwl:id>GAZ:00119101</oboInOwl:id>
        <rdfs:label>Santa Rosa District</rdfs:label>
    </owl:NamedIndividual>
    


    <!-- http://purl.obolibrary.org/obo/GAZ_00119102 -->

    <owl:NamedIndividual rdf:about="http://purl.obolibrary.org/obo/GAZ_00119102">
        <rdf:type rdf:resource="http://purl.obolibrary.org/obo/ENVO_00000004"/>
        <obo:RO_0001025 rdf:resource="http://purl.obolibrary.org/obo/GAZ_00068707"/>
        <obo:IAO_0000115>A district of Santo Domingo Canton.</obo:IAO_0000115>
        <oboInOwl:hasOBONamespace>GAZ</oboInOwl:hasOBONamespace>
        <oboInOwl:id>GAZ:00119102</oboInOwl:id>
        <rdfs:label>Paracito District</rdfs:label>
    </owl:NamedIndividual>
    


    <!-- http://purl.obolibrary.org/obo/GAZ_00119103 -->

    <owl:NamedIndividual rdf:about="http://purl.obolibrary.org/obo/GAZ_00119103">
        <rdf:type rdf:resource="http://purl.obolibrary.org/obo/ENVO_00000004"/>
        <obo:RO_0001025 rdf:resource="http://purl.obolibrary.org/obo/GAZ_00068707"/>
        <obo:IAO_0000115>A district of Santo Domingo Canton.</obo:IAO_0000115>
        <oboInOwl:hasOBONamespace>GAZ</oboInOwl:hasOBONamespace>
        <oboInOwl:id>GAZ:00119103</oboInOwl:id>
        <rdfs:label>San Miguel District</rdfs:label>
    </owl:NamedIndividual>
    


    <!-- http://purl.obolibrary.org/obo/GAZ_00119104 -->

    <owl:NamedIndividual rdf:about="http://purl.obolibrary.org/obo/GAZ_00119104">
        <rdf:type rdf:resource="http://purl.obolibrary.org/obo/ENVO_00000004"/>
        <obo:RO_0001025 rdf:resource="http://purl.obolibrary.org/obo/GAZ_00068707"/>
        <obo:IAO_0000115>A district of Santo Domingo Canton.</obo:IAO_0000115>
        <oboInOwl:hasOBONamespace>GAZ</oboInOwl:hasOBONamespace>
        <oboInOwl:id>GAZ:00119104</oboInOwl:id>
        <rdfs:label>Santo Domingo District</rdfs:label>
    </owl:NamedIndividual>
    


    <!-- http://purl.obolibrary.org/obo/GAZ_00119105 -->

    <owl:NamedIndividual rdf:about="http://purl.obolibrary.org/obo/GAZ_00119105">
        <rdf:type rdf:resource="http://purl.obolibrary.org/obo/ENVO_00000004"/>
        <obo:RO_0001025 rdf:resource="http://purl.obolibrary.org/obo/GAZ_00068706"/>
        <obo:IAO_0000115>A district of Santa Barbara Canton.</obo:IAO_0000115>
        <oboInOwl:hasOBONamespace>GAZ</oboInOwl:hasOBONamespace>
        <oboInOwl:id>GAZ:00119105</oboInOwl:id>
        <rdfs:label>San Juan District</rdfs:label>
    </owl:NamedIndividual>
    


    <!-- http://purl.obolibrary.org/obo/GAZ_00119106 -->

    <owl:NamedIndividual rdf:about="http://purl.obolibrary.org/obo/GAZ_00119106">
        <rdf:type rdf:resource="http://purl.obolibrary.org/obo/ENVO_00000004"/>
        <obo:RO_0001025 rdf:resource="http://purl.obolibrary.org/obo/GAZ_00068706"/>
        <obo:IAO_0000115>A district of Santa Barbara Canton.</obo:IAO_0000115>
        <oboInOwl:hasOBONamespace>GAZ</oboInOwl:hasOBONamespace>
        <oboInOwl:id>GAZ:00119106</oboInOwl:id>
        <rdfs:label>Jesus District</rdfs:label>
    </owl:NamedIndividual>
    


    <!-- http://purl.obolibrary.org/obo/GAZ_00119107 -->

    <owl:NamedIndividual rdf:about="http://purl.obolibrary.org/obo/GAZ_00119107">
        <rdf:type rdf:resource="http://purl.obolibrary.org/obo/ENVO_00000004"/>
        <obo:RO_0001025 rdf:resource="http://purl.obolibrary.org/obo/GAZ_00068706"/>
        <obo:IAO_0000115>A district of Santa Barbara Canton.</obo:IAO_0000115>
        <oboInOwl:hasOBONamespace>GAZ</oboInOwl:hasOBONamespace>
        <oboInOwl:id>GAZ:00119107</oboInOwl:id>
        <rdfs:label>Santa Barbara District</rdfs:label>
    </owl:NamedIndividual>
    


    <!-- http://purl.obolibrary.org/obo/GAZ_00119108 -->

    <owl:NamedIndividual rdf:about="http://purl.obolibrary.org/obo/GAZ_00119108">
        <rdf:type rdf:resource="http://purl.obolibrary.org/obo/ENVO_00000004"/>
        <obo:RO_0001025 rdf:resource="http://purl.obolibrary.org/obo/GAZ_00068706"/>
        <obo:IAO_0000115>A district of Santa Barbara Canton.</obo:IAO_0000115>
        <oboInOwl:hasOBONamespace>GAZ</oboInOwl:hasOBONamespace>
        <oboInOwl:id>GAZ:00119108</oboInOwl:id>
        <rdfs:label>San Pedro District</rdfs:label>
    </owl:NamedIndividual>
    


    <!-- http://purl.obolibrary.org/obo/GAZ_00119109 -->

    <owl:NamedIndividual rdf:about="http://purl.obolibrary.org/obo/GAZ_00119109">
        <rdf:type rdf:resource="http://purl.obolibrary.org/obo/ENVO_00000004"/>
        <obo:RO_0001025 rdf:resource="http://purl.obolibrary.org/obo/GAZ_00068706"/>
        <obo:IAO_0000115>A district of Santa Barbara Canton.</obo:IAO_0000115>
        <oboInOwl:hasOBONamespace>GAZ</oboInOwl:hasOBONamespace>
        <oboInOwl:id>GAZ:00119109</oboInOwl:id>
        <rdfs:label>Puraba District</rdfs:label>
    </owl:NamedIndividual>
    


    <!-- http://purl.obolibrary.org/obo/GAZ_00119110 -->

    <owl:NamedIndividual rdf:about="http://purl.obolibrary.org/obo/GAZ_00119110">
        <rdf:type rdf:resource="http://purl.obolibrary.org/obo/ENVO_00000004"/>
        <obo:RO_0001025 rdf:resource="http://purl.obolibrary.org/obo/GAZ_00068706"/>
        <obo:IAO_0000115>A district of Santa Barbara Canton.</obo:IAO_0000115>
        <oboInOwl:hasOBONamespace>GAZ</oboInOwl:hasOBONamespace>
        <oboInOwl:id>GAZ:00119110</oboInOwl:id>
        <rdfs:label>Santo Domingo District</rdfs:label>
    </owl:NamedIndividual>
    


    <!-- http://purl.obolibrary.org/obo/GAZ_00119111 -->

    <owl:NamedIndividual rdf:about="http://purl.obolibrary.org/obo/GAZ_00119111">
        <rdf:type rdf:resource="http://purl.obolibrary.org/obo/ENVO_00000004"/>
        <obo:RO_0001025 rdf:resource="http://purl.obolibrary.org/obo/GAZ_00068705"/>
        <obo:IAO_0000115>A district of San Rafael Canton.</obo:IAO_0000115>
        <oboInOwl:hasOBONamespace>GAZ</oboInOwl:hasOBONamespace>
        <oboInOwl:id>GAZ:00119111</oboInOwl:id>
        <rdfs:label>San Rafael District</rdfs:label>
    </owl:NamedIndividual>
    


    <!-- http://purl.obolibrary.org/obo/GAZ_00119112 -->

    <owl:NamedIndividual rdf:about="http://purl.obolibrary.org/obo/GAZ_00119112">
        <rdf:type rdf:resource="http://purl.obolibrary.org/obo/ENVO_00000004"/>
        <obo:RO_0001025 rdf:resource="http://purl.obolibrary.org/obo/GAZ_00068705"/>
        <obo:IAO_0000115>A district of San Rafael Canton.</obo:IAO_0000115>
        <oboInOwl:hasOBONamespace>GAZ</oboInOwl:hasOBONamespace>
        <oboInOwl:id>GAZ:00119112</oboInOwl:id>
        <rdfs:label>Santiago District</rdfs:label>
    </owl:NamedIndividual>
    


    <!-- http://purl.obolibrary.org/obo/GAZ_00119113 -->

    <owl:NamedIndividual rdf:about="http://purl.obolibrary.org/obo/GAZ_00119113">
        <rdf:type rdf:resource="http://purl.obolibrary.org/obo/ENVO_00000004"/>
        <obo:RO_0001025 rdf:resource="http://purl.obolibrary.org/obo/GAZ_00068705"/>
        <obo:IAO_0000115>A district of San Rafael Canton.</obo:IAO_0000115>
        <oboInOwl:hasOBONamespace>GAZ</oboInOwl:hasOBONamespace>
        <oboInOwl:id>GAZ:00119113</oboInOwl:id>
        <rdfs:label>Concepcio District</rdfs:label>
    </owl:NamedIndividual>
    


    <!-- http://purl.obolibrary.org/obo/GAZ_00119114 -->

    <owl:NamedIndividual rdf:about="http://purl.obolibrary.org/obo/GAZ_00119114">
        <rdf:type rdf:resource="http://purl.obolibrary.org/obo/ENVO_00000004"/>
        <obo:RO_0001025 rdf:resource="http://purl.obolibrary.org/obo/GAZ_00068705"/>
        <obo:IAO_0000115>A district of San Rafael Canton.</obo:IAO_0000115>
        <oboInOwl:hasOBONamespace>GAZ</oboInOwl:hasOBONamespace>
        <oboInOwl:id>GAZ:00119114</oboInOwl:id>
        <rdfs:label>Los Angeles District</rdfs:label>
    </owl:NamedIndividual>
    


    <!-- http://purl.obolibrary.org/obo/GAZ_00119115 -->

    <owl:NamedIndividual rdf:about="http://purl.obolibrary.org/obo/GAZ_00119115">
        <rdf:type rdf:resource="http://purl.obolibrary.org/obo/ENVO_00000004"/>
        <obo:RO_0001025 rdf:resource="http://purl.obolibrary.org/obo/GAZ_00068705"/>
        <obo:IAO_0000115>A district of San Rafael Canton.</obo:IAO_0000115>
        <oboInOwl:hasOBONamespace>GAZ</oboInOwl:hasOBONamespace>
        <oboInOwl:id>GAZ:00119115</oboInOwl:id>
        <rdfs:label>San Josecito District</rdfs:label>
    </owl:NamedIndividual>
    


    <!-- http://purl.obolibrary.org/obo/GAZ_00119116 -->

    <owl:NamedIndividual rdf:about="http://purl.obolibrary.org/obo/GAZ_00119116">
        <rdf:type rdf:resource="http://purl.obolibrary.org/obo/ENVO_00000004"/>
        <obo:RO_0001025 rdf:resource="http://purl.obolibrary.org/obo/GAZ_00068679"/>
        <obo:IAO_0000115>A district of Belen Canton.</obo:IAO_0000115>
        <oboInOwl:hasOBONamespace>GAZ</oboInOwl:hasOBONamespace>
        <oboInOwl:id>GAZ:00119116</oboInOwl:id>
        <rdfs:label>La Asuncion District</rdfs:label>
    </owl:NamedIndividual>
    


    <!-- http://purl.obolibrary.org/obo/GAZ_00119117 -->

    <owl:NamedIndividual rdf:about="http://purl.obolibrary.org/obo/GAZ_00119117">
        <rdf:type rdf:resource="http://purl.obolibrary.org/obo/ENVO_00000004"/>
        <obo:RO_0001025 rdf:resource="http://purl.obolibrary.org/obo/GAZ_00068679"/>
        <obo:IAO_0000115>A district of Belen Canton.</obo:IAO_0000115>
        <oboInOwl:hasOBONamespace>GAZ</oboInOwl:hasOBONamespace>
        <oboInOwl:id>GAZ:00119117</oboInOwl:id>
        <rdfs:label>San Antonio District</rdfs:label>
    </owl:NamedIndividual>
    


    <!-- http://purl.obolibrary.org/obo/GAZ_00119118 -->

    <owl:NamedIndividual rdf:about="http://purl.obolibrary.org/obo/GAZ_00119118">
        <rdf:type rdf:resource="http://purl.obolibrary.org/obo/ENVO_00000004"/>
        <obo:RO_0001025 rdf:resource="http://purl.obolibrary.org/obo/GAZ_00068679"/>
        <obo:IAO_0000115>A district of Belen Canton.</obo:IAO_0000115>
        <oboInOwl:hasOBONamespace>GAZ</oboInOwl:hasOBONamespace>
        <oboInOwl:id>GAZ:00119118</oboInOwl:id>
        <rdfs:label>La Ribera District</rdfs:label>
    </owl:NamedIndividual>
    


    <!-- http://purl.obolibrary.org/obo/GAZ_00119119 -->

    <owl:NamedIndividual rdf:about="http://purl.obolibrary.org/obo/GAZ_00119119">
        <rdf:type rdf:resource="http://purl.obolibrary.org/obo/ENVO_00000004"/>
        <obo:RO_0001025 rdf:resource="http://purl.obolibrary.org/obo/GAZ_00068704"/>
        <obo:IAO_0000115>A district of Flores Canton.</obo:IAO_0000115>
        <oboInOwl:hasOBONamespace>GAZ</oboInOwl:hasOBONamespace>
        <oboInOwl:id>GAZ:00119119</oboInOwl:id>
        <rdfs:label>Barrantes District</rdfs:label>
    </owl:NamedIndividual>
    


    <!-- http://purl.obolibrary.org/obo/GAZ_00119120 -->

    <owl:NamedIndividual rdf:about="http://purl.obolibrary.org/obo/GAZ_00119120">
        <rdf:type rdf:resource="http://purl.obolibrary.org/obo/ENVO_00000004"/>
        <obo:RO_0001025 rdf:resource="http://purl.obolibrary.org/obo/GAZ_00068704"/>
        <obo:IAO_0000115>A district of Flores Canton.</obo:IAO_0000115>
        <oboInOwl:hasOBONamespace>GAZ</oboInOwl:hasOBONamespace>
        <oboInOwl:id>GAZ:00119120</oboInOwl:id>
        <rdfs:label>San Joaquin District</rdfs:label>
    </owl:NamedIndividual>
    


    <!-- http://purl.obolibrary.org/obo/GAZ_00119121 -->

    <owl:NamedIndividual rdf:about="http://purl.obolibrary.org/obo/GAZ_00119121">
        <rdf:type rdf:resource="http://purl.obolibrary.org/obo/ENVO_00000004"/>
        <obo:RO_0001025 rdf:resource="http://purl.obolibrary.org/obo/GAZ_00068704"/>
        <obo:IAO_0000115>A district of Flores Canton.</obo:IAO_0000115>
        <oboInOwl:hasOBONamespace>GAZ</oboInOwl:hasOBONamespace>
        <oboInOwl:id>GAZ:00119121</oboInOwl:id>
        <rdfs:label>Llorente District</rdfs:label>
    </owl:NamedIndividual>
    


    <!-- http://purl.obolibrary.org/obo/GAZ_00119122 -->

    <owl:NamedIndividual rdf:about="http://purl.obolibrary.org/obo/GAZ_00119122">
        <rdf:type rdf:resource="http://purl.obolibrary.org/obo/ENVO_00000004"/>
        <obo:RO_0001025 rdf:resource="http://purl.obolibrary.org/obo/GAZ_00068680"/>
        <obo:IAO_0000115>A district of Sarapiqui Canton.</obo:IAO_0000115>
        <oboInOwl:hasOBONamespace>GAZ</oboInOwl:hasOBONamespace>
        <oboInOwl:id>GAZ:00119122</oboInOwl:id>
        <rdfs:label>Llanuras del Gaspar District</rdfs:label>
    </owl:NamedIndividual>
    


    <!-- http://purl.obolibrary.org/obo/GAZ_00119123 -->

    <owl:NamedIndividual rdf:about="http://purl.obolibrary.org/obo/GAZ_00119123">
        <rdf:type rdf:resource="http://purl.obolibrary.org/obo/ENVO_00000004"/>
        <obo:RO_0001025 rdf:resource="http://purl.obolibrary.org/obo/GAZ_00068680"/>
        <obo:IAO_0000115>A district of Sarapiqui Canton.</obo:IAO_0000115>
        <oboInOwl:hasOBONamespace>GAZ</oboInOwl:hasOBONamespace>
        <oboInOwl:id>GAZ:00119123</oboInOwl:id>
        <rdfs:label>Puerto Viejo District</rdfs:label>
    </owl:NamedIndividual>
    


    <!-- http://purl.obolibrary.org/obo/GAZ_00119124 -->

    <owl:NamedIndividual rdf:about="http://purl.obolibrary.org/obo/GAZ_00119124">
        <rdf:type rdf:resource="http://purl.obolibrary.org/obo/ENVO_00000004"/>
        <obo:RO_0001025 rdf:resource="http://purl.obolibrary.org/obo/GAZ_00068680"/>
        <obo:IAO_0000115>A district of Sarapiqui Canton.</obo:IAO_0000115>
        <oboInOwl:hasOBONamespace>GAZ</oboInOwl:hasOBONamespace>
        <oboInOwl:id>GAZ:00119124</oboInOwl:id>
        <rdfs:label>Las Horquetas District</rdfs:label>
    </owl:NamedIndividual>
    


    <!-- http://purl.obolibrary.org/obo/GAZ_00119125 -->

    <owl:NamedIndividual rdf:about="http://purl.obolibrary.org/obo/GAZ_00119125">
        <rdf:type rdf:resource="http://purl.obolibrary.org/obo/ENVO_00000004"/>
        <obo:RO_0001025 rdf:resource="http://purl.obolibrary.org/obo/GAZ_00068680"/>
        <obo:IAO_0000115>A district of Sarapiqui Canton.</obo:IAO_0000115>
        <oboInOwl:hasOBONamespace>GAZ</oboInOwl:hasOBONamespace>
        <oboInOwl:id>GAZ:00119125</oboInOwl:id>
        <rdfs:label>La Virgen District</rdfs:label>
    </owl:NamedIndividual>
    


    <!-- http://purl.obolibrary.org/obo/GAZ_00119126 -->

    <owl:NamedIndividual rdf:about="http://purl.obolibrary.org/obo/GAZ_00119126">
        <rdf:type rdf:resource="http://purl.obolibrary.org/obo/ENVO_00000004"/>
        <obo:RO_0001025 rdf:resource="http://purl.obolibrary.org/obo/GAZ_00068680"/>
        <obo:IAO_0000115>A district of Sarapiqui Canton.</obo:IAO_0000115>
        <oboInOwl:hasOBONamespace>GAZ</oboInOwl:hasOBONamespace>
        <oboInOwl:id>GAZ:00119126</oboInOwl:id>
        <rdfs:label>Curena District</rdfs:label>
    </owl:NamedIndividual>
    


    <!-- http://purl.obolibrary.org/obo/GAZ_00119127 -->

    <owl:NamedIndividual rdf:about="http://purl.obolibrary.org/obo/GAZ_00119127">
        <rdf:type rdf:resource="http://purl.obolibrary.org/obo/ENVO_00000004"/>
        <obo:RO_0001025 rdf:resource="http://purl.obolibrary.org/obo/GAZ_00068718"/>
        <obo:IAO_0000115>A district of Matina Canton.</obo:IAO_0000115>
        <oboInOwl:hasOBONamespace>GAZ</oboInOwl:hasOBONamespace>
        <oboInOwl:id>GAZ:00119127</oboInOwl:id>
        <rdfs:label>Matina District</rdfs:label>
    </owl:NamedIndividual>
    


    <!-- http://purl.obolibrary.org/obo/GAZ_00119128 -->

    <owl:NamedIndividual rdf:about="http://purl.obolibrary.org/obo/GAZ_00119128">
        <rdf:type rdf:resource="http://purl.obolibrary.org/obo/ENVO_00000004"/>
        <obo:RO_0001025 rdf:resource="http://purl.obolibrary.org/obo/GAZ_00068718"/>
        <obo:IAO_0000115>A district of Matina Canton.</obo:IAO_0000115>
        <oboInOwl:hasOBONamespace>GAZ</oboInOwl:hasOBONamespace>
        <oboInOwl:id>GAZ:00119128</oboInOwl:id>
        <rdfs:label>Batan District</rdfs:label>
    </owl:NamedIndividual>
    


    <!-- http://purl.obolibrary.org/obo/GAZ_00119129 -->

    <owl:NamedIndividual rdf:about="http://purl.obolibrary.org/obo/GAZ_00119129">
        <rdf:type rdf:resource="http://purl.obolibrary.org/obo/ENVO_00000004"/>
        <obo:RO_0001025 rdf:resource="http://purl.obolibrary.org/obo/GAZ_00068718"/>
        <obo:IAO_0000115>A district of Matina Canton.</obo:IAO_0000115>
        <oboInOwl:hasOBONamespace>GAZ</oboInOwl:hasOBONamespace>
        <oboInOwl:id>GAZ:00119129</oboInOwl:id>
        <rdfs:label>Carrandi District</rdfs:label>
    </owl:NamedIndividual>
    


    <!-- http://purl.obolibrary.org/obo/GAZ_00119130 -->

    <owl:NamedIndividual rdf:about="http://purl.obolibrary.org/obo/GAZ_00119130">
        <rdf:type rdf:resource="http://purl.obolibrary.org/obo/ENVO_00000004"/>
        <obo:RO_0001025 rdf:resource="http://purl.obolibrary.org/obo/GAZ_00068722"/>
        <obo:IAO_0000115>A district of Pococi Canton.</obo:IAO_0000115>
        <oboInOwl:hasOBONamespace>GAZ</oboInOwl:hasOBONamespace>
        <oboInOwl:id>GAZ:00119130</oboInOwl:id>
        <rdfs:label>Colorado District</rdfs:label>
    </owl:NamedIndividual>
    


    <!-- http://purl.obolibrary.org/obo/GAZ_00119131 -->

    <owl:NamedIndividual rdf:about="http://purl.obolibrary.org/obo/GAZ_00119131">
        <rdf:type rdf:resource="http://purl.obolibrary.org/obo/ENVO_00000004"/>
        <obo:RO_0001025 rdf:resource="http://purl.obolibrary.org/obo/GAZ_00068722"/>
        <obo:IAO_0000115>A district of Pococi Canton.</obo:IAO_0000115>
        <oboInOwl:hasOBONamespace>GAZ</oboInOwl:hasOBONamespace>
        <oboInOwl:id>GAZ:00119131</oboInOwl:id>
        <rdfs:label>Guapiles District</rdfs:label>
    </owl:NamedIndividual>
    


    <!-- http://purl.obolibrary.org/obo/GAZ_00119132 -->

    <owl:NamedIndividual rdf:about="http://purl.obolibrary.org/obo/GAZ_00119132">
        <rdf:type rdf:resource="http://purl.obolibrary.org/obo/ENVO_00000004"/>
        <obo:RO_0001025 rdf:resource="http://purl.obolibrary.org/obo/GAZ_00068722"/>
        <obo:IAO_0000115>A district of Pococi Canton.</obo:IAO_0000115>
        <oboInOwl:hasOBONamespace>GAZ</oboInOwl:hasOBONamespace>
        <oboInOwl:id>GAZ:00119132</oboInOwl:id>
        <rdfs:label>La Rita District</rdfs:label>
    </owl:NamedIndividual>
    


    <!-- http://purl.obolibrary.org/obo/GAZ_00119133 -->

    <owl:NamedIndividual rdf:about="http://purl.obolibrary.org/obo/GAZ_00119133">
        <rdf:type rdf:resource="http://purl.obolibrary.org/obo/ENVO_00000004"/>
        <obo:RO_0001025 rdf:resource="http://purl.obolibrary.org/obo/GAZ_00068722"/>
        <obo:IAO_0000115>A district of Pococi Canton.</obo:IAO_0000115>
        <oboInOwl:hasOBONamespace>GAZ</oboInOwl:hasOBONamespace>
        <oboInOwl:id>GAZ:00119133</oboInOwl:id>
        <rdfs:label>Roxana District</rdfs:label>
    </owl:NamedIndividual>
    


    <!-- http://purl.obolibrary.org/obo/GAZ_00119134 -->

    <owl:NamedIndividual rdf:about="http://purl.obolibrary.org/obo/GAZ_00119134">
        <rdf:type rdf:resource="http://purl.obolibrary.org/obo/ENVO_00000004"/>
        <obo:RO_0001025 rdf:resource="http://purl.obolibrary.org/obo/GAZ_00068722"/>
        <obo:IAO_0000115>A district of Pococi Canton.</obo:IAO_0000115>
        <oboInOwl:hasOBONamespace>GAZ</oboInOwl:hasOBONamespace>
        <oboInOwl:id>GAZ:00119134</oboInOwl:id>
        <rdfs:label>Cariari District</rdfs:label>
    </owl:NamedIndividual>
    


    <!-- http://purl.obolibrary.org/obo/GAZ_00119135 -->

    <owl:NamedIndividual rdf:about="http://purl.obolibrary.org/obo/GAZ_00119135">
        <rdf:type rdf:resource="http://purl.obolibrary.org/obo/ENVO_00000004"/>
        <obo:RO_0001025 rdf:resource="http://purl.obolibrary.org/obo/GAZ_00068722"/>
        <obo:IAO_0000115>A district of Pococi Canton.</obo:IAO_0000115>
        <oboInOwl:hasOBONamespace>GAZ</oboInOwl:hasOBONamespace>
        <oboInOwl:id>GAZ:00119135</oboInOwl:id>
        <rdfs:label>Jimenez District</rdfs:label>
    </owl:NamedIndividual>
    


    <!-- http://purl.obolibrary.org/obo/GAZ_00119136 -->

    <owl:NamedIndividual rdf:about="http://purl.obolibrary.org/obo/GAZ_00119136">
        <rdf:type rdf:resource="http://purl.obolibrary.org/obo/ENVO_00000004"/>
        <obo:RO_0001025 rdf:resource="http://purl.obolibrary.org/obo/GAZ_00068721"/>
        <obo:IAO_0000115>A district of Talamanca Canton.</obo:IAO_0000115>
        <oboInOwl:hasOBONamespace>GAZ</oboInOwl:hasOBONamespace>
        <oboInOwl:id>GAZ:00119136</oboInOwl:id>
        <rdfs:label>Bratsi District</rdfs:label>
    </owl:NamedIndividual>
    


    <!-- http://purl.obolibrary.org/obo/GAZ_00119137 -->

    <owl:NamedIndividual rdf:about="http://purl.obolibrary.org/obo/GAZ_00119137">
        <rdf:type rdf:resource="http://purl.obolibrary.org/obo/ENVO_00000004"/>
        <obo:RO_0001025 rdf:resource="http://purl.obolibrary.org/obo/GAZ_00068721"/>
        <obo:IAO_0000115>A district of Talamanca Canton.</obo:IAO_0000115>
        <oboInOwl:hasOBONamespace>GAZ</oboInOwl:hasOBONamespace>
        <oboInOwl:id>GAZ:00119137</oboInOwl:id>
        <rdfs:label>Sixaola District</rdfs:label>
    </owl:NamedIndividual>
    


    <!-- http://purl.obolibrary.org/obo/GAZ_00119138 -->

    <owl:NamedIndividual rdf:about="http://purl.obolibrary.org/obo/GAZ_00119138">
        <rdf:type rdf:resource="http://purl.obolibrary.org/obo/ENVO_00000004"/>
        <obo:RO_0001025 rdf:resource="http://purl.obolibrary.org/obo/GAZ_00068721"/>
        <obo:IAO_0000115>A district of Talamanca Canton.</obo:IAO_0000115>
        <oboInOwl:hasOBONamespace>GAZ</oboInOwl:hasOBONamespace>
        <oboInOwl:id>GAZ:00119138</oboInOwl:id>
        <rdfs:label>Cahuita Dsitrict</rdfs:label>
    </owl:NamedIndividual>
    


    <!-- http://purl.obolibrary.org/obo/GAZ_00119139 -->

    <owl:NamedIndividual rdf:about="http://purl.obolibrary.org/obo/GAZ_00119139">
        <rdf:type rdf:resource="http://purl.obolibrary.org/obo/ENVO_00000004"/>
        <obo:RO_0001025 rdf:resource="http://purl.obolibrary.org/obo/GAZ_00068720"/>
        <obo:IAO_0000115>A district of Limon Canton.</obo:IAO_0000115>
        <oboInOwl:hasOBONamespace>GAZ</oboInOwl:hasOBONamespace>
        <oboInOwl:id>GAZ:00119139</oboInOwl:id>
        <rdfs:label>Rio Blanco District</rdfs:label>
    </owl:NamedIndividual>
    


    <!-- http://purl.obolibrary.org/obo/GAZ_00119140 -->

    <owl:NamedIndividual rdf:about="http://purl.obolibrary.org/obo/GAZ_00119140">
        <rdf:type rdf:resource="http://purl.obolibrary.org/obo/ENVO_00000004"/>
        <obo:RO_0001025 rdf:resource="http://purl.obolibrary.org/obo/GAZ_00068720"/>
        <obo:IAO_0000115>A district of Limon Canton.</obo:IAO_0000115>
        <oboInOwl:hasOBONamespace>GAZ</oboInOwl:hasOBONamespace>
        <oboInOwl:id>GAZ:00119140</oboInOwl:id>
        <rdfs:label>Valle La Estrella District</rdfs:label>
    </owl:NamedIndividual>
    


    <!-- http://purl.obolibrary.org/obo/GAZ_00119141 -->

    <owl:NamedIndividual rdf:about="http://purl.obolibrary.org/obo/GAZ_00119141">
        <rdf:type rdf:resource="http://purl.obolibrary.org/obo/ENVO_00000004"/>
        <obo:RO_0001025 rdf:resource="http://purl.obolibrary.org/obo/GAZ_00068720"/>
        <obo:IAO_0000115>A district of Limon Canton.</obo:IAO_0000115>
        <oboInOwl:hasOBONamespace>GAZ</oboInOwl:hasOBONamespace>
        <oboInOwl:id>GAZ:00119141</oboInOwl:id>
        <rdfs:label>Matama District</rdfs:label>
    </owl:NamedIndividual>
    


    <!-- http://purl.obolibrary.org/obo/GAZ_00119142 -->

    <owl:NamedIndividual rdf:about="http://purl.obolibrary.org/obo/GAZ_00119142">
        <rdf:type rdf:resource="http://purl.obolibrary.org/obo/ENVO_00000004"/>
        <obo:RO_0001025 rdf:resource="http://purl.obolibrary.org/obo/GAZ_00068720"/>
        <obo:IAO_0000115>A district of Limon Canton.</obo:IAO_0000115>
        <oboInOwl:hasOBONamespace>GAZ</oboInOwl:hasOBONamespace>
        <oboInOwl:id>GAZ:00119142</oboInOwl:id>
        <rdfs:label>Limon City District</rdfs:label>
    </owl:NamedIndividual>
    


    <!-- http://purl.obolibrary.org/obo/GAZ_00119143 -->

    <owl:NamedIndividual rdf:about="http://purl.obolibrary.org/obo/GAZ_00119143">
        <rdf:type rdf:resource="http://purl.obolibrary.org/obo/ENVO_00000004"/>
        <obo:RO_0001025 rdf:resource="http://purl.obolibrary.org/obo/GAZ_00068701"/>
        <obo:IAO_0000115>A district of Guacimo Canton.</obo:IAO_0000115>
        <oboInOwl:hasOBONamespace>GAZ</oboInOwl:hasOBONamespace>
        <oboInOwl:id>GAZ:00119143</oboInOwl:id>
        <rdfs:label>Guacimo City District</rdfs:label>
    </owl:NamedIndividual>
    


    <!-- http://purl.obolibrary.org/obo/GAZ_00119144 -->

    <owl:NamedIndividual rdf:about="http://purl.obolibrary.org/obo/GAZ_00119144">
        <rdf:type rdf:resource="http://purl.obolibrary.org/obo/ENVO_00000004"/>
        <obo:RO_0001025 rdf:resource="http://purl.obolibrary.org/obo/GAZ_00068701"/>
        <obo:IAO_0000115>A district of Guacimo Canton.</obo:IAO_0000115>
        <oboInOwl:hasOBONamespace>GAZ</oboInOwl:hasOBONamespace>
        <oboInOwl:id>GAZ:00119144</oboInOwl:id>
        <rdfs:label>Pocora District</rdfs:label>
    </owl:NamedIndividual>
    


    <!-- http://purl.obolibrary.org/obo/GAZ_00119145 -->

    <owl:NamedIndividual rdf:about="http://purl.obolibrary.org/obo/GAZ_00119145">
        <rdf:type rdf:resource="http://purl.obolibrary.org/obo/ENVO_00000004"/>
        <obo:RO_0001025 rdf:resource="http://purl.obolibrary.org/obo/GAZ_00068701"/>
        <obo:IAO_0000115>A district of Guacimo Canton.</obo:IAO_0000115>
        <oboInOwl:hasOBONamespace>GAZ</oboInOwl:hasOBONamespace>
        <oboInOwl:id>GAZ:00119145</oboInOwl:id>
        <rdfs:label>Duacari District</rdfs:label>
    </owl:NamedIndividual>
    


    <!-- http://purl.obolibrary.org/obo/GAZ_00119146 -->

    <owl:NamedIndividual rdf:about="http://purl.obolibrary.org/obo/GAZ_00119146">
        <rdf:type rdf:resource="http://purl.obolibrary.org/obo/ENVO_00000004"/>
        <obo:RO_0001025 rdf:resource="http://purl.obolibrary.org/obo/GAZ_00068701"/>
        <obo:IAO_0000115>A district of Guacimo Canton.</obo:IAO_0000115>
        <oboInOwl:hasOBONamespace>GAZ</oboInOwl:hasOBONamespace>
        <oboInOwl:id>GAZ:00119146</oboInOwl:id>
        <rdfs:label>Mercedes District</rdfs:label>
    </owl:NamedIndividual>
    


    <!-- http://purl.obolibrary.org/obo/GAZ_00119147 -->

    <owl:NamedIndividual rdf:about="http://purl.obolibrary.org/obo/GAZ_00119147">
        <rdf:type rdf:resource="http://purl.obolibrary.org/obo/ENVO_00000004"/>
        <obo:RO_0001025 rdf:resource="http://purl.obolibrary.org/obo/GAZ_00068701"/>
        <obo:IAO_0000115>A district of Guacimo Canton.</obo:IAO_0000115>
        <oboInOwl:hasOBONamespace>GAZ</oboInOwl:hasOBONamespace>
        <oboInOwl:id>GAZ:00119147</oboInOwl:id>
        <rdfs:label>Rio Jimenez District</rdfs:label>
    </owl:NamedIndividual>
    


    <!-- http://purl.obolibrary.org/obo/GAZ_00119148 -->

    <owl:NamedIndividual rdf:about="http://purl.obolibrary.org/obo/GAZ_00119148">
        <rdf:type rdf:resource="http://purl.obolibrary.org/obo/ENVO_00000004"/>
        <obo:RO_0001025 rdf:resource="http://purl.obolibrary.org/obo/GAZ_00068719"/>
        <obo:IAO_0000115>A district of Siquirres Canton.</obo:IAO_0000115>
        <oboInOwl:hasOBONamespace>GAZ</oboInOwl:hasOBONamespace>
        <oboInOwl:id>GAZ:00119148</oboInOwl:id>
        <rdfs:label>Siquirres City District</rdfs:label>
    </owl:NamedIndividual>
    


    <!-- http://purl.obolibrary.org/obo/GAZ_00119149 -->

    <owl:NamedIndividual rdf:about="http://purl.obolibrary.org/obo/GAZ_00119149">
        <rdf:type rdf:resource="http://purl.obolibrary.org/obo/ENVO_00000004"/>
        <obo:RO_0001025 rdf:resource="http://purl.obolibrary.org/obo/GAZ_00068719"/>
        <obo:IAO_0000115>A district of Siquirres Canton.</obo:IAO_0000115>
        <oboInOwl:hasOBONamespace>GAZ</oboInOwl:hasOBONamespace>
        <oboInOwl:id>GAZ:00119149</oboInOwl:id>
        <rdfs:label>Florida District</rdfs:label>
    </owl:NamedIndividual>
    


    <!-- http://purl.obolibrary.org/obo/GAZ_00119150 -->

    <owl:NamedIndividual rdf:about="http://purl.obolibrary.org/obo/GAZ_00119150">
        <rdf:type rdf:resource="http://purl.obolibrary.org/obo/ENVO_00000004"/>
        <obo:RO_0001025 rdf:resource="http://purl.obolibrary.org/obo/GAZ_00068719"/>
        <obo:IAO_0000115>A district of Siquirres Canton.</obo:IAO_0000115>
        <oboInOwl:hasOBONamespace>GAZ</oboInOwl:hasOBONamespace>
        <oboInOwl:id>GAZ:00119150</oboInOwl:id>
        <rdfs:label>Cairo District</rdfs:label>
    </owl:NamedIndividual>
    


    <!-- http://purl.obolibrary.org/obo/GAZ_00119151 -->

    <owl:NamedIndividual rdf:about="http://purl.obolibrary.org/obo/GAZ_00119151">
        <rdf:type rdf:resource="http://purl.obolibrary.org/obo/ENVO_00000004"/>
        <obo:RO_0001025 rdf:resource="http://purl.obolibrary.org/obo/GAZ_00068719"/>
        <obo:IAO_0000115>A district of Siquirres Canton.</obo:IAO_0000115>
        <oboInOwl:hasOBONamespace>GAZ</oboInOwl:hasOBONamespace>
        <oboInOwl:id>GAZ:00119151</oboInOwl:id>
        <rdfs:label>Germania District</rdfs:label>
    </owl:NamedIndividual>
    


    <!-- http://purl.obolibrary.org/obo/GAZ_00119152 -->

    <owl:NamedIndividual rdf:about="http://purl.obolibrary.org/obo/GAZ_00119152">
        <rdf:type rdf:resource="http://purl.obolibrary.org/obo/ENVO_00000004"/>
        <obo:RO_0001025 rdf:resource="http://purl.obolibrary.org/obo/GAZ_00068719"/>
        <obo:IAO_0000115>A district of Siquirres Canton.</obo:IAO_0000115>
        <oboInOwl:hasOBONamespace>GAZ</oboInOwl:hasOBONamespace>
        <oboInOwl:id>GAZ:00119152</oboInOwl:id>
        <rdfs:label>Pacuarito District</rdfs:label>
    </owl:NamedIndividual>
    


    <!-- http://purl.obolibrary.org/obo/GAZ_00119153 -->

    <owl:NamedIndividual rdf:about="http://purl.obolibrary.org/obo/GAZ_00119153">
        <rdf:type rdf:resource="http://purl.obolibrary.org/obo/ENVO_00000004"/>
        <obo:RO_0001025 rdf:resource="http://purl.obolibrary.org/obo/GAZ_00068719"/>
        <obo:IAO_0000115>A district of Siquirres Canton.</obo:IAO_0000115>
        <oboInOwl:hasOBONamespace>GAZ</oboInOwl:hasOBONamespace>
        <oboInOwl:id>GAZ:00119153</oboInOwl:id>
        <rdfs:label>La Alegria District</rdfs:label>
    </owl:NamedIndividual>
    


    <!-- http://purl.obolibrary.org/obo/GAZ_00119154 -->

    <owl:NamedIndividual rdf:about="http://purl.obolibrary.org/obo/GAZ_00119154">
        <rdf:type rdf:resource="http://purl.obolibrary.org/obo/ENVO_00000004"/>
        <obo:RO_0001025 rdf:resource="http://purl.obolibrary.org/obo/GAZ_00068734"/>
        <obo:IAO_0000115>A district of Aguirre Canton.</obo:IAO_0000115>
        <oboInOwl:hasOBONamespace>GAZ</oboInOwl:hasOBONamespace>
        <oboInOwl:id>GAZ:00119154</oboInOwl:id>
        <rdfs:label>Savegre District</rdfs:label>
    </owl:NamedIndividual>
    


    <!-- http://purl.obolibrary.org/obo/GAZ_00119155 -->

    <owl:NamedIndividual rdf:about="http://purl.obolibrary.org/obo/GAZ_00119155">
        <rdf:type rdf:resource="http://purl.obolibrary.org/obo/ENVO_00000004"/>
        <obo:RO_0001025 rdf:resource="http://purl.obolibrary.org/obo/GAZ_00068734"/>
        <obo:IAO_0000115>A district of Aguirre Canton.</obo:IAO_0000115>
        <oboInOwl:hasOBONamespace>GAZ</oboInOwl:hasOBONamespace>
        <oboInOwl:id>GAZ:00119155</oboInOwl:id>
        <rdfs:label>Naranjito District</rdfs:label>
    </owl:NamedIndividual>
    


    <!-- http://purl.obolibrary.org/obo/GAZ_00119156 -->

    <owl:NamedIndividual rdf:about="http://purl.obolibrary.org/obo/GAZ_00119156">
        <rdf:type rdf:resource="http://purl.obolibrary.org/obo/ENVO_00000004"/>
        <obo:RO_0001025 rdf:resource="http://purl.obolibrary.org/obo/GAZ_00068734"/>
        <obo:IAO_0000115>A district of Aguirre Canton.</obo:IAO_0000115>
        <oboInOwl:hasOBONamespace>GAZ</oboInOwl:hasOBONamespace>
        <oboInOwl:id>GAZ:00119156</oboInOwl:id>
        <rdfs:label>Quepos District</rdfs:label>
    </owl:NamedIndividual>
    


    <!-- http://purl.obolibrary.org/obo/GAZ_00119157 -->

    <owl:NamedIndividual rdf:about="http://purl.obolibrary.org/obo/GAZ_00119157">
        <rdf:type rdf:resource="http://purl.obolibrary.org/obo/ENVO_00000004"/>
        <obo:RO_0001025 rdf:resource="http://purl.obolibrary.org/obo/GAZ_00068729"/>
        <obo:IAO_0000115>A district of Buenos Aires Canton.</obo:IAO_0000115>
        <oboInOwl:hasOBONamespace>GAZ</oboInOwl:hasOBONamespace>
        <oboInOwl:id>GAZ:00119157</oboInOwl:id>
        <rdfs:label>Brunka District</rdfs:label>
    </owl:NamedIndividual>
    


    <!-- http://purl.obolibrary.org/obo/GAZ_00119158 -->

    <owl:NamedIndividual rdf:about="http://purl.obolibrary.org/obo/GAZ_00119158">
        <rdf:type rdf:resource="http://purl.obolibrary.org/obo/ENVO_00000004"/>
        <obo:RO_0001025 rdf:resource="http://purl.obolibrary.org/obo/GAZ_00068729"/>
        <obo:IAO_0000115>A district of Buenos Aires Canton.</obo:IAO_0000115>
        <oboInOwl:hasOBONamespace>GAZ</oboInOwl:hasOBONamespace>
        <oboInOwl:id>GAZ:00119158</oboInOwl:id>
        <rdfs:label>Pilas District</rdfs:label>
    </owl:NamedIndividual>
    


    <!-- http://purl.obolibrary.org/obo/GAZ_00119159 -->

    <owl:NamedIndividual rdf:about="http://purl.obolibrary.org/obo/GAZ_00119159">
        <rdf:type rdf:resource="http://purl.obolibrary.org/obo/ENVO_00000004"/>
        <obo:RO_0001025 rdf:resource="http://purl.obolibrary.org/obo/GAZ_00068729"/>
        <obo:IAO_0000115>A district of Buenos Aires Canton.</obo:IAO_0000115>
        <oboInOwl:hasOBONamespace>GAZ</oboInOwl:hasOBONamespace>
        <oboInOwl:id>GAZ:00119159</oboInOwl:id>
        <rdfs:label>Changuena District</rdfs:label>
    </owl:NamedIndividual>
    


    <!-- http://purl.obolibrary.org/obo/GAZ_00119160 -->

    <owl:NamedIndividual rdf:about="http://purl.obolibrary.org/obo/GAZ_00119160">
        <rdf:type rdf:resource="http://purl.obolibrary.org/obo/ENVO_00000004"/>
        <obo:RO_0001025 rdf:resource="http://purl.obolibrary.org/obo/GAZ_00068729"/>
        <obo:IAO_0000115>A district of Buenos Aires Canton.</obo:IAO_0000115>
        <oboInOwl:hasOBONamespace>GAZ</oboInOwl:hasOBONamespace>
        <oboInOwl:id>GAZ:00119160</oboInOwl:id>
        <rdfs:label>Boruca District</rdfs:label>
    </owl:NamedIndividual>
    


    <!-- http://purl.obolibrary.org/obo/GAZ_00119161 -->

    <owl:NamedIndividual rdf:about="http://purl.obolibrary.org/obo/GAZ_00119161">
        <rdf:type rdf:resource="http://purl.obolibrary.org/obo/ENVO_00000004"/>
        <obo:RO_0001025 rdf:resource="http://purl.obolibrary.org/obo/GAZ_00068729"/>
        <obo:IAO_0000115>A district of Buenos Aires Canton.</obo:IAO_0000115>
        <oboInOwl:hasOBONamespace>GAZ</oboInOwl:hasOBONamespace>
        <oboInOwl:id>GAZ:00119161</oboInOwl:id>
        <rdfs:label>Biolley District</rdfs:label>
    </owl:NamedIndividual>
    


    <!-- http://purl.obolibrary.org/obo/GAZ_00119162 -->

    <owl:NamedIndividual rdf:about="http://purl.obolibrary.org/obo/GAZ_00119162">
        <rdf:type rdf:resource="http://purl.obolibrary.org/obo/ENVO_00000004"/>
        <obo:RO_0001025 rdf:resource="http://purl.obolibrary.org/obo/GAZ_00068729"/>
        <obo:IAO_0000115>A district of Buenos Aires Canton.</obo:IAO_0000115>
        <oboInOwl:hasOBONamespace>GAZ</oboInOwl:hasOBONamespace>
        <oboInOwl:id>GAZ:00119162</oboInOwl:id>
        <rdfs:label>Colinas District</rdfs:label>
    </owl:NamedIndividual>
    


    <!-- http://purl.obolibrary.org/obo/GAZ_00119163 -->

    <owl:NamedIndividual rdf:about="http://purl.obolibrary.org/obo/GAZ_00119163">
        <rdf:type rdf:resource="http://purl.obolibrary.org/obo/ENVO_00000004"/>
        <obo:RO_0001025 rdf:resource="http://purl.obolibrary.org/obo/GAZ_00068729"/>
        <obo:IAO_0000115>A district of Buenos Aires Canton.</obo:IAO_0000115>
        <oboInOwl:hasOBONamespace>GAZ</oboInOwl:hasOBONamespace>
        <oboInOwl:id>GAZ:00119163</oboInOwl:id>
        <rdfs:label>Potrero Grande District</rdfs:label>
    </owl:NamedIndividual>
    


    <!-- http://purl.obolibrary.org/obo/GAZ_00119164 -->

    <owl:NamedIndividual rdf:about="http://purl.obolibrary.org/obo/GAZ_00119164">
        <rdf:type rdf:resource="http://purl.obolibrary.org/obo/ENVO_00000004"/>
        <obo:RO_0001025 rdf:resource="http://purl.obolibrary.org/obo/GAZ_00068729"/>
        <obo:IAO_0000115>A district of Buenos Aires Canton.</obo:IAO_0000115>
        <oboInOwl:hasOBONamespace>GAZ</oboInOwl:hasOBONamespace>
        <oboInOwl:id>GAZ:00119164</oboInOwl:id>
        <rdfs:label>Volcan District</rdfs:label>
    </owl:NamedIndividual>
    


    <!-- http://purl.obolibrary.org/obo/GAZ_00119165 -->

    <owl:NamedIndividual rdf:about="http://purl.obolibrary.org/obo/GAZ_00119165">
        <rdf:type rdf:resource="http://purl.obolibrary.org/obo/ENVO_00000004"/>
        <obo:RO_0001025 rdf:resource="http://purl.obolibrary.org/obo/GAZ_00068729"/>
        <obo:IAO_0000115>A district of Buenos Aires Canton.</obo:IAO_0000115>
        <oboInOwl:hasOBONamespace>GAZ</oboInOwl:hasOBONamespace>
        <oboInOwl:id>GAZ:00119165</oboInOwl:id>
        <rdfs:label>Buenos Aires District</rdfs:label>
    </owl:NamedIndividual>
    


    <!-- http://purl.obolibrary.org/obo/GAZ_00119166 -->

    <owl:NamedIndividual rdf:about="http://purl.obolibrary.org/obo/GAZ_00119166">
        <rdf:type rdf:resource="http://purl.obolibrary.org/obo/ENVO_00000004"/>
        <obo:RO_0001025 rdf:resource="http://purl.obolibrary.org/obo/GAZ_00068728"/>
        <obo:IAO_0000115>A district of Corredores Canton.</obo:IAO_0000115>
        <oboInOwl:hasOBONamespace>GAZ</oboInOwl:hasOBONamespace>
        <oboInOwl:id>GAZ:00119166</oboInOwl:id>
        <rdfs:label>La Cuesta District</rdfs:label>
    </owl:NamedIndividual>
    


    <!-- http://purl.obolibrary.org/obo/GAZ_00119167 -->

    <owl:NamedIndividual rdf:about="http://purl.obolibrary.org/obo/GAZ_00119167">
        <rdf:type rdf:resource="http://purl.obolibrary.org/obo/ENVO_00000004"/>
        <obo:RO_0001025 rdf:resource="http://purl.obolibrary.org/obo/GAZ_00068728"/>
        <obo:IAO_0000115>A district of Corredores Canton.</obo:IAO_0000115>
        <oboInOwl:hasOBONamespace>GAZ</oboInOwl:hasOBONamespace>
        <oboInOwl:id>GAZ:00119167</oboInOwl:id>
        <rdfs:label>Corredor District</rdfs:label>
    </owl:NamedIndividual>
    


    <!-- http://purl.obolibrary.org/obo/GAZ_00119168 -->

    <owl:NamedIndividual rdf:about="http://purl.obolibrary.org/obo/GAZ_00119168">
        <rdf:type rdf:resource="http://purl.obolibrary.org/obo/ENVO_00000004"/>
        <obo:RO_0001025 rdf:resource="http://purl.obolibrary.org/obo/GAZ_00068728"/>
        <obo:IAO_0000115>A district of Corredores Canton.</obo:IAO_0000115>
        <oboInOwl:hasOBONamespace>GAZ</oboInOwl:hasOBONamespace>
        <oboInOwl:id>GAZ:00119168</oboInOwl:id>
        <rdfs:label>Laurel District</rdfs:label>
    </owl:NamedIndividual>
    


    <!-- http://purl.obolibrary.org/obo/GAZ_00119169 -->

    <owl:NamedIndividual rdf:about="http://purl.obolibrary.org/obo/GAZ_00119169">
        <rdf:type rdf:resource="http://purl.obolibrary.org/obo/ENVO_00000004"/>
        <obo:RO_0001025 rdf:resource="http://purl.obolibrary.org/obo/GAZ_00068728"/>
        <obo:IAO_0000115>A district of Corredores Canton.</obo:IAO_0000115>
        <oboInOwl:hasOBONamespace>GAZ</oboInOwl:hasOBONamespace>
        <oboInOwl:id>GAZ:00119169</oboInOwl:id>
        <rdfs:label>Canoas District</rdfs:label>
    </owl:NamedIndividual>
    


    <!-- http://purl.obolibrary.org/obo/GAZ_00119170 -->

    <owl:NamedIndividual rdf:about="http://purl.obolibrary.org/obo/GAZ_00119170">
        <rdf:type rdf:resource="http://purl.obolibrary.org/obo/ENVO_00000004"/>
        <obo:RO_0001025 rdf:resource="http://purl.obolibrary.org/obo/GAZ_00003212"/>
        <obo:IAO_0000115>A district of Coto Brus Canton.</obo:IAO_0000115>
        <oboInOwl:hasOBONamespace>GAZ</oboInOwl:hasOBONamespace>
        <oboInOwl:id>GAZ:00119170</oboInOwl:id>
        <rdfs:label>San Vito District</rdfs:label>
    </owl:NamedIndividual>
    


    <!-- http://purl.obolibrary.org/obo/GAZ_00119171 -->

    <owl:NamedIndividual rdf:about="http://purl.obolibrary.org/obo/GAZ_00119171">
        <rdf:type rdf:resource="http://purl.obolibrary.org/obo/ENVO_00000004"/>
        <obo:RO_0001025 rdf:resource="http://purl.obolibrary.org/obo/GAZ_00003212"/>
        <obo:IAO_0000115>A district of Coto Brus Canton.</obo:IAO_0000115>
        <oboInOwl:hasOBONamespace>GAZ</oboInOwl:hasOBONamespace>
        <oboInOwl:id>GAZ:00119171</oboInOwl:id>
        <rdfs:label>Pittier District</rdfs:label>
    </owl:NamedIndividual>
    


    <!-- http://purl.obolibrary.org/obo/GAZ_00119172 -->

    <owl:NamedIndividual rdf:about="http://purl.obolibrary.org/obo/GAZ_00119172">
        <rdf:type rdf:resource="http://purl.obolibrary.org/obo/ENVO_00000004"/>
        <obo:RO_0001025 rdf:resource="http://purl.obolibrary.org/obo/GAZ_00003212"/>
        <obo:IAO_0000115>A district of Coto Brus Canton.</obo:IAO_0000115>
        <oboInOwl:hasOBONamespace>GAZ</oboInOwl:hasOBONamespace>
        <oboInOwl:id>GAZ:00119172</oboInOwl:id>
        <rdfs:label>Agua Buena District</rdfs:label>
    </owl:NamedIndividual>
    


    <!-- http://purl.obolibrary.org/obo/GAZ_00119173 -->

    <owl:NamedIndividual rdf:about="http://purl.obolibrary.org/obo/GAZ_00119173">
        <rdf:type rdf:resource="http://purl.obolibrary.org/obo/ENVO_00000004"/>
        <obo:RO_0001025 rdf:resource="http://purl.obolibrary.org/obo/GAZ_00003212"/>
        <obo:IAO_0000115>A district of Coto Brus Canton.</obo:IAO_0000115>
        <oboInOwl:hasOBONamespace>GAZ</oboInOwl:hasOBONamespace>
        <oboInOwl:id>GAZ:00119173</oboInOwl:id>
        <rdfs:label>Sabalito District</rdfs:label>
    </owl:NamedIndividual>
    


    <!-- http://purl.obolibrary.org/obo/GAZ_00119174 -->

    <owl:NamedIndividual rdf:about="http://purl.obolibrary.org/obo/GAZ_00119174">
        <rdf:type rdf:resource="http://purl.obolibrary.org/obo/ENVO_00000004"/>
        <obo:RO_0001025 rdf:resource="http://purl.obolibrary.org/obo/GAZ_00003212"/>
        <obo:IAO_0000115>A district of Coto Brus Canton.</obo:IAO_0000115>
        <oboInOwl:hasOBONamespace>GAZ</oboInOwl:hasOBONamespace>
        <oboInOwl:id>GAZ:00119174</oboInOwl:id>
        <rdfs:label>Limoncito District</rdfs:label>
    </owl:NamedIndividual>
    


    <!-- http://purl.obolibrary.org/obo/GAZ_00119175 -->

    <owl:NamedIndividual rdf:about="http://purl.obolibrary.org/obo/GAZ_00119175">
        <rdf:type rdf:resource="http://purl.obolibrary.org/obo/ENVO_00000004"/>
        <obo:RO_0001025 rdf:resource="http://purl.obolibrary.org/obo/GAZ_00068731"/>
        <obo:IAO_0000115>A district of Esparza Canton.</obo:IAO_0000115>
        <oboInOwl:hasOBONamespace>GAZ</oboInOwl:hasOBONamespace>
        <oboInOwl:id>GAZ:00119175</oboInOwl:id>
        <rdfs:label>San Juan Grande District</rdfs:label>
    </owl:NamedIndividual>
    


    <!-- http://purl.obolibrary.org/obo/GAZ_00119176 -->

    <owl:NamedIndividual rdf:about="http://purl.obolibrary.org/obo/GAZ_00119176">
        <rdf:type rdf:resource="http://purl.obolibrary.org/obo/ENVO_00000004"/>
        <obo:RO_0001025 rdf:resource="http://purl.obolibrary.org/obo/GAZ_00068731"/>
        <obo:IAO_0000115>A district of Esparza Canton.</obo:IAO_0000115>
        <oboInOwl:hasOBONamespace>GAZ</oboInOwl:hasOBONamespace>
        <oboInOwl:id>GAZ:00119176</oboInOwl:id>
        <rdfs:label>Macacona District</rdfs:label>
    </owl:NamedIndividual>
    


    <!-- http://purl.obolibrary.org/obo/GAZ_00119177 -->

    <owl:NamedIndividual rdf:about="http://purl.obolibrary.org/obo/GAZ_00119177">
        <rdf:type rdf:resource="http://purl.obolibrary.org/obo/ENVO_00000004"/>
        <obo:RO_0001025 rdf:resource="http://purl.obolibrary.org/obo/GAZ_00068731"/>
        <obo:IAO_0000115>A district of Esparza Canton.</obo:IAO_0000115>
        <oboInOwl:hasOBONamespace>GAZ</oboInOwl:hasOBONamespace>
        <oboInOwl:id>GAZ:00119177</oboInOwl:id>
        <rdfs:label>San Jeronimo District</rdfs:label>
    </owl:NamedIndividual>
    


    <!-- http://purl.obolibrary.org/obo/GAZ_00119178 -->

    <owl:NamedIndividual rdf:about="http://purl.obolibrary.org/obo/GAZ_00119178">
        <rdf:type rdf:resource="http://purl.obolibrary.org/obo/ENVO_00000004"/>
        <obo:RO_0001025 rdf:resource="http://purl.obolibrary.org/obo/GAZ_00068731"/>
        <obo:IAO_0000115>A district of Esparza Canton.</obo:IAO_0000115>
        <oboInOwl:hasOBONamespace>GAZ</oboInOwl:hasOBONamespace>
        <oboInOwl:id>GAZ:00119178</oboInOwl:id>
        <rdfs:label>San Rafael District</rdfs:label>
    </owl:NamedIndividual>
    


    <!-- http://purl.obolibrary.org/obo/GAZ_00119179 -->

    <owl:NamedIndividual rdf:about="http://purl.obolibrary.org/obo/GAZ_00119179">
        <rdf:type rdf:resource="http://purl.obolibrary.org/obo/ENVO_00000004"/>
        <obo:RO_0001025 rdf:resource="http://purl.obolibrary.org/obo/GAZ_00068731"/>
        <obo:IAO_0000115>A district of Esparza Canton.</obo:IAO_0000115>
        <oboInOwl:hasOBONamespace>GAZ</oboInOwl:hasOBONamespace>
        <oboInOwl:id>GAZ:00119179</oboInOwl:id>
        <rdfs:label>Espiritu Santo District</rdfs:label>
    </owl:NamedIndividual>
    


    <!-- http://purl.obolibrary.org/obo/GAZ_00119180 -->

    <owl:NamedIndividual rdf:about="http://purl.obolibrary.org/obo/GAZ_00119180">
        <rdf:type rdf:resource="http://purl.obolibrary.org/obo/ENVO_00000004"/>
        <obo:RO_0001025 rdf:resource="http://purl.obolibrary.org/obo/GAZ_00068730"/>
        <obo:IAO_0000115>A district of Garabito Canton.</obo:IAO_0000115>
        <oboInOwl:hasOBONamespace>GAZ</oboInOwl:hasOBONamespace>
        <oboInOwl:id>GAZ:00119180</oboInOwl:id>
        <rdfs:label>Jaco District</rdfs:label>
    </owl:NamedIndividual>
    


    <!-- http://purl.obolibrary.org/obo/GAZ_00119181 -->

    <owl:NamedIndividual rdf:about="http://purl.obolibrary.org/obo/GAZ_00119181">
        <rdf:type rdf:resource="http://purl.obolibrary.org/obo/ENVO_00000004"/>
        <obo:RO_0001025 rdf:resource="http://purl.obolibrary.org/obo/GAZ_00068730"/>
        <obo:IAO_0000115>A district of Garabito Canton.</obo:IAO_0000115>
        <oboInOwl:hasOBONamespace>GAZ</oboInOwl:hasOBONamespace>
        <oboInOwl:id>GAZ:00119181</oboInOwl:id>
        <rdfs:label>Tarcoles District</rdfs:label>
    </owl:NamedIndividual>
    


    <!-- http://purl.obolibrary.org/obo/GAZ_00119182 -->

    <owl:NamedIndividual rdf:about="http://purl.obolibrary.org/obo/GAZ_00119182">
        <rdf:type rdf:resource="http://purl.obolibrary.org/obo/ENVO_00000004"/>
        <obo:RO_0001025 rdf:resource="http://purl.obolibrary.org/obo/GAZ_00068732"/>
        <obo:IAO_0000115>A district of Montes de Oro Canton.</obo:IAO_0000115>
        <oboInOwl:hasOBONamespace>GAZ</oboInOwl:hasOBONamespace>
        <oboInOwl:id>GAZ:00119182</oboInOwl:id>
        <rdfs:label>Miramar District</rdfs:label>
    </owl:NamedIndividual>
    


    <!-- http://purl.obolibrary.org/obo/GAZ_00119183 -->

    <owl:NamedIndividual rdf:about="http://purl.obolibrary.org/obo/GAZ_00119183">
        <rdf:type rdf:resource="http://purl.obolibrary.org/obo/ENVO_00000004"/>
        <obo:RO_0001025 rdf:resource="http://purl.obolibrary.org/obo/GAZ_00068732"/>
        <obo:IAO_0000115>A district of Montes de Oro Canton.</obo:IAO_0000115>
        <oboInOwl:hasOBONamespace>GAZ</oboInOwl:hasOBONamespace>
        <oboInOwl:id>GAZ:00119183</oboInOwl:id>
        <rdfs:label>La Union District</rdfs:label>
    </owl:NamedIndividual>
    


    <!-- http://purl.obolibrary.org/obo/GAZ_00119184 -->

    <owl:NamedIndividual rdf:about="http://purl.obolibrary.org/obo/GAZ_00119184">
        <rdf:type rdf:resource="http://purl.obolibrary.org/obo/ENVO_00000004"/>
        <obo:RO_0001025 rdf:resource="http://purl.obolibrary.org/obo/GAZ_00068732"/>
        <obo:IAO_0000115>A district of Montes de Oro Canton.</obo:IAO_0000115>
        <oboInOwl:hasOBONamespace>GAZ</oboInOwl:hasOBONamespace>
        <oboInOwl:id>GAZ:00119184</oboInOwl:id>
        <rdfs:label>San Isidro District</rdfs:label>
    </owl:NamedIndividual>
    


    <!-- http://purl.obolibrary.org/obo/GAZ_00119185 -->

    <owl:NamedIndividual rdf:about="http://purl.obolibrary.org/obo/GAZ_00119185">
        <rdf:type rdf:resource="http://purl.obolibrary.org/obo/ENVO_00000004"/>
        <obo:RO_0001025 rdf:resource="http://purl.obolibrary.org/obo/GAZ_00068727"/>
        <obo:IAO_0000115>A district of Osa Canton.</obo:IAO_0000115>
        <oboInOwl:hasOBONamespace>GAZ</oboInOwl:hasOBONamespace>
        <oboInOwl:id>GAZ:00119185</oboInOwl:id>
        <rdfs:label>Piedras Blancas District</rdfs:label>
    </owl:NamedIndividual>
    


    <!-- http://purl.obolibrary.org/obo/GAZ_00119186 -->

    <owl:NamedIndividual rdf:about="http://purl.obolibrary.org/obo/GAZ_00119186">
        <rdf:type rdf:resource="http://purl.obolibrary.org/obo/ENVO_00000004"/>
        <obo:RO_0001025 rdf:resource="http://purl.obolibrary.org/obo/GAZ_00068727"/>
        <obo:IAO_0000115>A district of Osa Canton.</obo:IAO_0000115>
        <oboInOwl:hasOBONamespace>GAZ</oboInOwl:hasOBONamespace>
        <oboInOwl:id>GAZ:00119186</oboInOwl:id>
        <rdfs:label>Bahia Ballena District</rdfs:label>
    </owl:NamedIndividual>
    


    <!-- http://purl.obolibrary.org/obo/GAZ_00119187 -->

    <owl:NamedIndividual rdf:about="http://purl.obolibrary.org/obo/GAZ_00119187">
        <rdf:type rdf:resource="http://purl.obolibrary.org/obo/ENVO_00000004"/>
        <obo:RO_0001025 rdf:resource="http://purl.obolibrary.org/obo/GAZ_00068727"/>
        <obo:IAO_0000115>A district of Osa Canton.</obo:IAO_0000115>
        <oboInOwl:hasOBONamespace>GAZ</oboInOwl:hasOBONamespace>
        <oboInOwl:id>GAZ:00119187</oboInOwl:id>
        <rdfs:label>Sierpe District</rdfs:label>
    </owl:NamedIndividual>
    


    <!-- http://purl.obolibrary.org/obo/GAZ_00119188 -->

    <owl:NamedIndividual rdf:about="http://purl.obolibrary.org/obo/GAZ_00119188">
        <rdf:type rdf:resource="http://purl.obolibrary.org/obo/ENVO_00000004"/>
        <obo:RO_0001025 rdf:resource="http://purl.obolibrary.org/obo/GAZ_00068727"/>
        <obo:IAO_0000115>A district of Osa Canton.</obo:IAO_0000115>
        <oboInOwl:hasOBONamespace>GAZ</oboInOwl:hasOBONamespace>
        <oboInOwl:id>GAZ:00119188</oboInOwl:id>
        <rdfs:label>Palmar District</rdfs:label>
    </owl:NamedIndividual>
    


    <!-- http://purl.obolibrary.org/obo/GAZ_00119189 -->

    <owl:NamedIndividual rdf:about="http://purl.obolibrary.org/obo/GAZ_00119189">
        <rdf:type rdf:resource="http://purl.obolibrary.org/obo/ENVO_00000004"/>
        <obo:RO_0001025 rdf:resource="http://purl.obolibrary.org/obo/GAZ_00068727"/>
        <obo:IAO_0000115>A district of Osa Canton.</obo:IAO_0000115>
        <oboInOwl:hasOBONamespace>GAZ</oboInOwl:hasOBONamespace>
        <oboInOwl:id>GAZ:00119189</oboInOwl:id>
        <rdfs:label>Cortes District</rdfs:label>
    </owl:NamedIndividual>
    


    <!-- http://purl.obolibrary.org/obo/GAZ_00119190 -->

    <owl:NamedIndividual rdf:about="http://purl.obolibrary.org/obo/GAZ_00119190">
        <rdf:type rdf:resource="http://purl.obolibrary.org/obo/ENVO_00000004"/>
        <obo:RO_0001025 rdf:resource="http://purl.obolibrary.org/obo/GAZ_00047498"/>
        <obo:IAO_0000115>A district of Puntarenas Canton.</obo:IAO_0000115>
        <oboInOwl:hasOBONamespace>GAZ</oboInOwl:hasOBONamespace>
        <oboInOwl:id>GAZ:00119190</oboInOwl:id>
        <rdfs:label>Isla de Coco District</rdfs:label>
    </owl:NamedIndividual>
    


    <!-- http://purl.obolibrary.org/obo/GAZ_00119191 -->

    <owl:NamedIndividual rdf:about="http://purl.obolibrary.org/obo/GAZ_00119191">
        <rdf:type rdf:resource="http://purl.obolibrary.org/obo/ENVO_00000004"/>
        <obo:RO_0001025 rdf:resource="http://purl.obolibrary.org/obo/GAZ_00047498"/>
        <obo:IAO_0000115>A district of Puntarenas Canton.</obo:IAO_0000115>
        <oboInOwl:hasOBONamespace>GAZ</oboInOwl:hasOBONamespace>
        <oboInOwl:id>GAZ:00119191</oboInOwl:id>
        <rdfs:label>Manzanillo District</rdfs:label>
    </owl:NamedIndividual>
    


    <!-- http://purl.obolibrary.org/obo/GAZ_00119192 -->

    <owl:NamedIndividual rdf:about="http://purl.obolibrary.org/obo/GAZ_00119192">
        <rdf:type rdf:resource="http://purl.obolibrary.org/obo/ENVO_00000004"/>
        <obo:RO_0001025 rdf:resource="http://purl.obolibrary.org/obo/GAZ_00047498"/>
        <obo:IAO_0000115>A district of Puntarenas Canton.</obo:IAO_0000115>
        <oboInOwl:hasOBONamespace>GAZ</oboInOwl:hasOBONamespace>
        <oboInOwl:id>GAZ:00119192</oboInOwl:id>
        <rdfs:label>Cobano District</rdfs:label>
    </owl:NamedIndividual>
    


    <!-- http://purl.obolibrary.org/obo/GAZ_00119193 -->

    <owl:NamedIndividual rdf:about="http://purl.obolibrary.org/obo/GAZ_00119193">
        <rdf:type rdf:resource="http://purl.obolibrary.org/obo/ENVO_00000004"/>
        <obo:RO_0001025 rdf:resource="http://purl.obolibrary.org/obo/GAZ_00047498"/>
        <obo:IAO_0000115>A district of Puntarenas Canton.</obo:IAO_0000115>
        <oboInOwl:hasOBONamespace>GAZ</oboInOwl:hasOBONamespace>
        <oboInOwl:id>GAZ:00119193</oboInOwl:id>
        <rdfs:label>Arancibia District</rdfs:label>
    </owl:NamedIndividual>
    


    <!-- http://purl.obolibrary.org/obo/GAZ_00119194 -->

    <owl:NamedIndividual rdf:about="http://purl.obolibrary.org/obo/GAZ_00119194">
        <rdf:type rdf:resource="http://purl.obolibrary.org/obo/ENVO_00000004"/>
        <obo:RO_0001025 rdf:resource="http://purl.obolibrary.org/obo/GAZ_00047498"/>
        <obo:IAO_0000115>A district of Puntarenas Canton.</obo:IAO_0000115>
        <oboInOwl:hasOBONamespace>GAZ</oboInOwl:hasOBONamespace>
        <oboInOwl:id>GAZ:00119194</oboInOwl:id>
        <rdfs:label>Lepanto District</rdfs:label>
    </owl:NamedIndividual>
    


    <!-- http://purl.obolibrary.org/obo/GAZ_00119195 -->

    <owl:NamedIndividual rdf:about="http://purl.obolibrary.org/obo/GAZ_00119195">
        <rdf:type rdf:resource="http://purl.obolibrary.org/obo/ENVO_00000004"/>
        <obo:RO_0001025 rdf:resource="http://purl.obolibrary.org/obo/GAZ_00047498"/>
        <obo:IAO_0000115>A district of Puntarenas Canton.</obo:IAO_0000115>
        <oboInOwl:hasOBONamespace>GAZ</oboInOwl:hasOBONamespace>
        <oboInOwl:id>GAZ:00119195</oboInOwl:id>
        <rdfs:label>Puntarenas District</rdfs:label>
    </owl:NamedIndividual>
    


    <!-- http://purl.obolibrary.org/obo/GAZ_00119196 -->

    <owl:NamedIndividual rdf:about="http://purl.obolibrary.org/obo/GAZ_00119196">
        <rdf:type rdf:resource="http://purl.obolibrary.org/obo/ENVO_00000004"/>
        <obo:RO_0001025 rdf:resource="http://purl.obolibrary.org/obo/GAZ_00047498"/>
        <obo:IAO_0000115>A district of Puntarenas Canton.</obo:IAO_0000115>
        <oboInOwl:hasOBONamespace>GAZ</oboInOwl:hasOBONamespace>
        <oboInOwl:id>GAZ:00119196</oboInOwl:id>
        <rdfs:label>Paquera District</rdfs:label>
    </owl:NamedIndividual>
    


    <!-- http://purl.obolibrary.org/obo/GAZ_00119197 -->

    <owl:NamedIndividual rdf:about="http://purl.obolibrary.org/obo/GAZ_00119197">
        <rdf:type rdf:resource="http://purl.obolibrary.org/obo/ENVO_00000004"/>
        <obo:RO_0001025 rdf:resource="http://purl.obolibrary.org/obo/GAZ_00047498"/>
        <obo:IAO_0000115>A district of Puntarenas Canton.</obo:IAO_0000115>
        <oboInOwl:hasOBONamespace>GAZ</oboInOwl:hasOBONamespace>
        <oboInOwl:id>GAZ:00119197</oboInOwl:id>
        <rdfs:label>Guacimal District</rdfs:label>
    </owl:NamedIndividual>
    


    <!-- http://purl.obolibrary.org/obo/GAZ_00119198 -->

    <owl:NamedIndividual rdf:about="http://purl.obolibrary.org/obo/GAZ_00119198">
        <rdf:type rdf:resource="http://purl.obolibrary.org/obo/ENVO_00000004"/>
        <obo:RO_0001025 rdf:resource="http://purl.obolibrary.org/obo/GAZ_00047498"/>
        <obo:IAO_0000115>A district of Puntarenas Canton.</obo:IAO_0000115>
        <oboInOwl:hasOBONamespace>GAZ</oboInOwl:hasOBONamespace>
        <oboInOwl:id>GAZ:00119198</oboInOwl:id>
        <rdfs:label>Chomes District</rdfs:label>
    </owl:NamedIndividual>
    


    <!-- http://purl.obolibrary.org/obo/GAZ_00119199 -->

    <owl:NamedIndividual rdf:about="http://purl.obolibrary.org/obo/GAZ_00119199">
        <rdf:type rdf:resource="http://purl.obolibrary.org/obo/ENVO_00000004"/>
        <obo:RO_0001025 rdf:resource="http://purl.obolibrary.org/obo/GAZ_00047498"/>
        <obo:IAO_0000115>A district of Puntarenas Canton.</obo:IAO_0000115>
        <oboInOwl:hasOBONamespace>GAZ</oboInOwl:hasOBONamespace>
        <oboInOwl:id>GAZ:00119199</oboInOwl:id>
        <rdfs:label>Pitahaya District</rdfs:label>
    </owl:NamedIndividual>
    


    <!-- http://purl.obolibrary.org/obo/GAZ_00119200 -->

    <owl:NamedIndividual rdf:about="http://purl.obolibrary.org/obo/GAZ_00119200">
        <rdf:type rdf:resource="http://purl.obolibrary.org/obo/ENVO_00000004"/>
        <obo:RO_0001025 rdf:resource="http://purl.obolibrary.org/obo/GAZ_00047498"/>
        <obo:IAO_0000115>A district of Puntarenas Canton.</obo:IAO_0000115>
        <oboInOwl:hasOBONamespace>GAZ</oboInOwl:hasOBONamespace>
        <oboInOwl:id>GAZ:00119200</oboInOwl:id>
        <rdfs:label>Acapulco District</rdfs:label>
    </owl:NamedIndividual>
    


    <!-- http://purl.obolibrary.org/obo/GAZ_00119201 -->

    <owl:NamedIndividual rdf:about="http://purl.obolibrary.org/obo/GAZ_00119201">
        <rdf:type rdf:resource="http://purl.obolibrary.org/obo/ENVO_00000004"/>
        <obo:RO_0001025 rdf:resource="http://purl.obolibrary.org/obo/GAZ_00047498"/>
        <obo:IAO_0000115>A district of Puntarenas Canton.</obo:IAO_0000115>
        <oboInOwl:hasOBONamespace>GAZ</oboInOwl:hasOBONamespace>
        <oboInOwl:id>GAZ:00119201</oboInOwl:id>
        <rdfs:label>Barranca District</rdfs:label>
    </owl:NamedIndividual>
    


    <!-- http://purl.obolibrary.org/obo/GAZ_00119202 -->

    <owl:NamedIndividual rdf:about="http://purl.obolibrary.org/obo/GAZ_00119202">
        <rdf:type rdf:resource="http://purl.obolibrary.org/obo/ENVO_00000004"/>
        <obo:RO_0001025 rdf:resource="http://purl.obolibrary.org/obo/GAZ_00047498"/>
        <obo:IAO_0000115>A district of Puntarenas Canton.</obo:IAO_0000115>
        <oboInOwl:hasOBONamespace>GAZ</oboInOwl:hasOBONamespace>
        <oboInOwl:id>GAZ:00119202</oboInOwl:id>
        <rdfs:label>Chacarita District</rdfs:label>
    </owl:NamedIndividual>
    


    <!-- http://purl.obolibrary.org/obo/GAZ_00119203 -->

    <owl:NamedIndividual rdf:about="http://purl.obolibrary.org/obo/GAZ_00119203">
        <rdf:type rdf:resource="http://purl.obolibrary.org/obo/ENVO_00000004"/>
        <obo:RO_0001025 rdf:resource="http://purl.obolibrary.org/obo/GAZ_00047498"/>
        <obo:IAO_0000115>A district of Puntarenas Canton.</obo:IAO_0000115>
        <oboInOwl:hasOBONamespace>GAZ</oboInOwl:hasOBONamespace>
        <oboInOwl:id>GAZ:00119203</oboInOwl:id>
        <rdfs:label>Isla Chira District</rdfs:label>
    </owl:NamedIndividual>
    


    <!-- http://purl.obolibrary.org/obo/GAZ_00119204 -->

    <owl:NamedIndividual rdf:about="http://purl.obolibrary.org/obo/GAZ_00119204">
        <rdf:type rdf:resource="http://purl.obolibrary.org/obo/ENVO_00000004"/>
        <obo:RO_0001025 rdf:resource="http://purl.obolibrary.org/obo/GAZ_00047498"/>
        <obo:IAO_0000115>A district of Puntarenas Canton.</obo:IAO_0000115>
        <oboInOwl:hasOBONamespace>GAZ</oboInOwl:hasOBONamespace>
        <oboInOwl:id>GAZ:00119204</oboInOwl:id>
        <rdfs:label>Monteverde District</rdfs:label>
    </owl:NamedIndividual>
    


    <!-- http://purl.obolibrary.org/obo/GAZ_00119205 -->

    <owl:NamedIndividual rdf:about="http://purl.obolibrary.org/obo/GAZ_00119205">
        <rdf:type rdf:resource="http://purl.obolibrary.org/obo/ENVO_00000004"/>
        <obo:RO_0001025 rdf:resource="http://purl.obolibrary.org/obo/GAZ_00047498"/>
        <obo:IAO_0000115>A district of Puntarenas Canton.</obo:IAO_0000115>
        <oboInOwl:hasOBONamespace>GAZ</oboInOwl:hasOBONamespace>
        <oboInOwl:id>GAZ:00119205</oboInOwl:id>
        <rdfs:label>El Roble District</rdfs:label>
    </owl:NamedIndividual>
    


    <!-- http://purl.obolibrary.org/obo/GAZ_00119212 -->

    <owl:NamedIndividual rdf:about="http://purl.obolibrary.org/obo/GAZ_00119212">
        <rdf:type rdf:resource="http://purl.obolibrary.org/obo/ENVO_00000004"/>
        <obo:RO_0001025 rdf:resource="http://purl.obolibrary.org/obo/GAZ_00068766"/>
        <obo:IAO_0000115>A district of Escazu Canton.</obo:IAO_0000115>
        <oboInOwl:hasOBONamespace>GAZ</oboInOwl:hasOBONamespace>
        <oboInOwl:id>GAZ:00119212</oboInOwl:id>
        <rdfs:label>San Miguel de Escazu District</rdfs:label>
    </owl:NamedIndividual>
    


    <!-- http://purl.obolibrary.org/obo/GAZ_00119213 -->

    <owl:NamedIndividual rdf:about="http://purl.obolibrary.org/obo/GAZ_00119213">
        <rdf:type rdf:resource="http://purl.obolibrary.org/obo/ENVO_00000004"/>
        <obo:RO_0001025 rdf:resource="http://purl.obolibrary.org/obo/GAZ_00068766"/>
        <obo:IAO_0000115>A district of Escazu Canton.</obo:IAO_0000115>
        <oboInOwl:hasOBONamespace>GAZ</oboInOwl:hasOBONamespace>
        <oboInOwl:id>GAZ:00119213</oboInOwl:id>
        <rdfs:label>San Antonio de Escazu District</rdfs:label>
    </owl:NamedIndividual>
    


    <!-- http://purl.obolibrary.org/obo/GAZ_00119214 -->

    <owl:NamedIndividual rdf:about="http://purl.obolibrary.org/obo/GAZ_00119214">
        <rdf:type rdf:resource="http://purl.obolibrary.org/obo/ENVO_00000004"/>
        <obo:RO_0001025 rdf:resource="http://purl.obolibrary.org/obo/GAZ_00068766"/>
        <obo:IAO_0000115>A district of Escazu Canton.</obo:IAO_0000115>
        <oboInOwl:hasOBONamespace>GAZ</oboInOwl:hasOBONamespace>
        <oboInOwl:id>GAZ:00119214</oboInOwl:id>
        <rdfs:label>San Rafael de Escazu District</rdfs:label>
    </owl:NamedIndividual>
    


    <!-- http://purl.obolibrary.org/obo/GAZ_00119215 -->

    <owl:NamedIndividual rdf:about="http://purl.obolibrary.org/obo/GAZ_00119215">
        <rdf:type rdf:resource="http://purl.obolibrary.org/obo/ENVO_00000004"/>
        <obo:RO_0001025 rdf:resource="http://purl.obolibrary.org/obo/GAZ_00068768"/>
        <obo:IAO_0000115>A district of Desamparados Canton.</obo:IAO_0000115>
        <oboInOwl:hasOBONamespace>GAZ</oboInOwl:hasOBONamespace>
        <oboInOwl:id>GAZ:00119215</oboInOwl:id>
        <rdfs:label>Gravilias de Desamparados District</rdfs:label>
    </owl:NamedIndividual>
    


    <!-- http://purl.obolibrary.org/obo/GAZ_00119216 -->

    <owl:NamedIndividual rdf:about="http://purl.obolibrary.org/obo/GAZ_00119216">
        <rdf:type rdf:resource="http://purl.obolibrary.org/obo/ENVO_00000004"/>
        <obo:RO_0001025 rdf:resource="http://purl.obolibrary.org/obo/GAZ_00068768"/>
        <obo:IAO_0000115>A district of Desamparados Canton.</obo:IAO_0000115>
        <oboInOwl:hasOBONamespace>GAZ</oboInOwl:hasOBONamespace>
        <oboInOwl:id>GAZ:00119216</oboInOwl:id>
        <rdfs:label>San Rafael Arriba District</rdfs:label>
    </owl:NamedIndividual>
    


    <!-- http://purl.obolibrary.org/obo/GAZ_00119217 -->

    <owl:NamedIndividual rdf:about="http://purl.obolibrary.org/obo/GAZ_00119217">
        <rdf:type rdf:resource="http://purl.obolibrary.org/obo/ENVO_00000004"/>
        <obo:RO_0001025 rdf:resource="http://purl.obolibrary.org/obo/GAZ_00068768"/>
        <obo:IAO_0000115>A district of Desamparados Canton.</obo:IAO_0000115>
        <oboInOwl:hasOBONamespace>GAZ</oboInOwl:hasOBONamespace>
        <oboInOwl:id>GAZ:00119217</oboInOwl:id>
        <rdfs:label>San Miguel District</rdfs:label>
    </owl:NamedIndividual>
    


    <!-- http://purl.obolibrary.org/obo/GAZ_00119218 -->

    <owl:NamedIndividual rdf:about="http://purl.obolibrary.org/obo/GAZ_00119218">
        <rdf:type rdf:resource="http://purl.obolibrary.org/obo/ENVO_00000004"/>
        <obo:RO_0001025 rdf:resource="http://purl.obolibrary.org/obo/GAZ_00068768"/>
        <obo:IAO_0000115>A district of Desamparados Canton.</obo:IAO_0000115>
        <oboInOwl:hasOBONamespace>GAZ</oboInOwl:hasOBONamespace>
        <oboInOwl:id>GAZ:00119218</oboInOwl:id>
        <rdfs:label>San Juan de Dios District</rdfs:label>
    </owl:NamedIndividual>
    


    <!-- http://purl.obolibrary.org/obo/GAZ_00119219 -->

    <owl:NamedIndividual rdf:about="http://purl.obolibrary.org/obo/GAZ_00119219">
        <rdf:type rdf:resource="http://purl.obolibrary.org/obo/ENVO_00000004"/>
        <obo:RO_0001025 rdf:resource="http://purl.obolibrary.org/obo/GAZ_00068768"/>
        <obo:IAO_0000115>A district of Desamparados Canton.</obo:IAO_0000115>
        <oboInOwl:hasOBONamespace>GAZ</oboInOwl:hasOBONamespace>
        <oboInOwl:id>GAZ:00119219</oboInOwl:id>
        <rdfs:label>San Antonio District</rdfs:label>
    </owl:NamedIndividual>
    


    <!-- http://purl.obolibrary.org/obo/GAZ_00119220 -->

    <owl:NamedIndividual rdf:about="http://purl.obolibrary.org/obo/GAZ_00119220">
        <rdf:type rdf:resource="http://purl.obolibrary.org/obo/ENVO_00000004"/>
        <obo:RO_0001025 rdf:resource="http://purl.obolibrary.org/obo/GAZ_00068768"/>
        <obo:IAO_0000115>A district of Desamparados Canton.</obo:IAO_0000115>
        <oboInOwl:hasOBONamespace>GAZ</oboInOwl:hasOBONamespace>
        <oboInOwl:id>GAZ:00119220</oboInOwl:id>
        <rdfs:label>Rosario District</rdfs:label>
    </owl:NamedIndividual>
    


    <!-- http://purl.obolibrary.org/obo/GAZ_00119221 -->

    <owl:NamedIndividual rdf:about="http://purl.obolibrary.org/obo/GAZ_00119221">
        <rdf:type rdf:resource="http://purl.obolibrary.org/obo/ENVO_00000004"/>
        <obo:RO_0001025 rdf:resource="http://purl.obolibrary.org/obo/GAZ_00068768"/>
        <obo:IAO_0000115>A district of Desamparados Canton.</obo:IAO_0000115>
        <oboInOwl:hasOBONamespace>GAZ</oboInOwl:hasOBONamespace>
        <oboInOwl:id>GAZ:00119221</oboInOwl:id>
        <rdfs:label>Damas District</rdfs:label>
    </owl:NamedIndividual>
    


    <!-- http://purl.obolibrary.org/obo/GAZ_00119222 -->

    <owl:NamedIndividual rdf:about="http://purl.obolibrary.org/obo/GAZ_00119222">
        <rdf:type rdf:resource="http://purl.obolibrary.org/obo/ENVO_00000004"/>
        <obo:RO_0001025 rdf:resource="http://purl.obolibrary.org/obo/GAZ_00068768"/>
        <obo:IAO_0000115>A district of Desamparados Canton.</obo:IAO_0000115>
        <oboInOwl:hasOBONamespace>GAZ</oboInOwl:hasOBONamespace>
        <oboInOwl:id>GAZ:00119222</oboInOwl:id>
        <rdfs:label>Patarra District</rdfs:label>
    </owl:NamedIndividual>
    


    <!-- http://purl.obolibrary.org/obo/GAZ_00119223 -->

    <owl:NamedIndividual rdf:about="http://purl.obolibrary.org/obo/GAZ_00119223">
        <rdf:type rdf:resource="http://purl.obolibrary.org/obo/ENVO_00000004"/>
        <obo:RO_0001025 rdf:resource="http://purl.obolibrary.org/obo/GAZ_00068768"/>
        <obo:IAO_0000115>A district of Desamparados Canton.</obo:IAO_0000115>
        <oboInOwl:hasOBONamespace>GAZ</oboInOwl:hasOBONamespace>
        <oboInOwl:id>GAZ:00119223</oboInOwl:id>
        <rdfs:label>Frailes District</rdfs:label>
    </owl:NamedIndividual>
    


    <!-- http://purl.obolibrary.org/obo/GAZ_00119224 -->

    <owl:NamedIndividual rdf:about="http://purl.obolibrary.org/obo/GAZ_00119224">
        <rdf:type rdf:resource="http://purl.obolibrary.org/obo/ENVO_00000004"/>
        <obo:RO_0001025 rdf:resource="http://purl.obolibrary.org/obo/GAZ_00068768"/>
        <obo:IAO_0000115>A district of Desamparados Canton.</obo:IAO_0000115>
        <oboInOwl:hasOBONamespace>GAZ</oboInOwl:hasOBONamespace>
        <oboInOwl:id>GAZ:00119224</oboInOwl:id>
        <rdfs:label>San Rafael Abajo District</rdfs:label>
    </owl:NamedIndividual>
    


    <!-- http://purl.obolibrary.org/obo/GAZ_00119225 -->

    <owl:NamedIndividual rdf:about="http://purl.obolibrary.org/obo/GAZ_00119225">
        <rdf:type rdf:resource="http://purl.obolibrary.org/obo/ENVO_00000004"/>
        <obo:RO_0001025 rdf:resource="http://purl.obolibrary.org/obo/GAZ_00068768"/>
        <obo:IAO_0000115>A district of Desamparados Canton.</obo:IAO_0000115>
        <oboInOwl:hasOBONamespace>GAZ</oboInOwl:hasOBONamespace>
        <oboInOwl:id>GAZ:00119225</oboInOwl:id>
        <rdfs:label>San Cristobal District</rdfs:label>
    </owl:NamedIndividual>
    


    <!-- http://purl.obolibrary.org/obo/GAZ_00119226 -->

    <owl:NamedIndividual rdf:about="http://purl.obolibrary.org/obo/GAZ_00119226">
        <rdf:type rdf:resource="http://purl.obolibrary.org/obo/ENVO_00000004"/>
        <obo:RO_0001025 rdf:resource="http://purl.obolibrary.org/obo/GAZ_00068768"/>
        <obo:IAO_0000115>A district of Desamparados Canton.</obo:IAO_0000115>
        <oboInOwl:hasOBONamespace>GAZ</oboInOwl:hasOBONamespace>
        <oboInOwl:id>GAZ:00119226</oboInOwl:id>
        <rdfs:label>Desamparados District</rdfs:label>
    </owl:NamedIndividual>
    


    <!-- http://purl.obolibrary.org/obo/GAZ_00119227 -->

    <owl:NamedIndividual rdf:about="http://purl.obolibrary.org/obo/GAZ_00119227">
        <rdf:type rdf:resource="http://purl.obolibrary.org/obo/ENVO_00000004"/>
        <obo:RO_0001025 rdf:resource="http://purl.obolibrary.org/obo/GAZ_00068781"/>
        <obo:IAO_0000115>A district of Puriscal Canton.</obo:IAO_0000115>
        <oboInOwl:hasOBONamespace>GAZ</oboInOwl:hasOBONamespace>
        <oboInOwl:id>GAZ:00119227</oboInOwl:id>
        <rdfs:label>Desamparaditos District</rdfs:label>
    </owl:NamedIndividual>
    


    <!-- http://purl.obolibrary.org/obo/GAZ_00119228 -->

    <owl:NamedIndividual rdf:about="http://purl.obolibrary.org/obo/GAZ_00119228">
        <rdf:type rdf:resource="http://purl.obolibrary.org/obo/ENVO_00000004"/>
        <obo:RO_0001025 rdf:resource="http://purl.obolibrary.org/obo/GAZ_00068781"/>
        <obo:IAO_0000115>A district of Puriscal Canton.</obo:IAO_0000115>
        <oboInOwl:hasOBONamespace>GAZ</oboInOwl:hasOBONamespace>
        <oboInOwl:id>GAZ:00119228</oboInOwl:id>
        <rdfs:label>Barbacoas District</rdfs:label>
    </owl:NamedIndividual>
    


    <!-- http://purl.obolibrary.org/obo/GAZ_00119229 -->

    <owl:NamedIndividual rdf:about="http://purl.obolibrary.org/obo/GAZ_00119229">
        <rdf:type rdf:resource="http://purl.obolibrary.org/obo/ENVO_00000004"/>
        <obo:RO_0001025 rdf:resource="http://purl.obolibrary.org/obo/GAZ_00068781"/>
        <obo:IAO_0000115>A district of Puriscal Canton.</obo:IAO_0000115>
        <oboInOwl:hasOBONamespace>GAZ</oboInOwl:hasOBONamespace>
        <oboInOwl:id>GAZ:00119229</oboInOwl:id>
        <rdfs:label>Santiago District</rdfs:label>
    </owl:NamedIndividual>
    


    <!-- http://purl.obolibrary.org/obo/GAZ_00119230 -->

    <owl:NamedIndividual rdf:about="http://purl.obolibrary.org/obo/GAZ_00119230">
        <rdf:type rdf:resource="http://purl.obolibrary.org/obo/ENVO_00000004"/>
        <obo:RO_0001025 rdf:resource="http://purl.obolibrary.org/obo/GAZ_00068781"/>
        <obo:IAO_0000115>A district of Puriscal Canton.</obo:IAO_0000115>
        <oboInOwl:hasOBONamespace>GAZ</oboInOwl:hasOBONamespace>
        <oboInOwl:id>GAZ:00119230</oboInOwl:id>
        <rdfs:label>Mercedes Sur District</rdfs:label>
    </owl:NamedIndividual>
    


    <!-- http://purl.obolibrary.org/obo/GAZ_00119231 -->

    <owl:NamedIndividual rdf:about="http://purl.obolibrary.org/obo/GAZ_00119231">
        <rdf:type rdf:resource="http://purl.obolibrary.org/obo/ENVO_00000004"/>
        <obo:RO_0001025 rdf:resource="http://purl.obolibrary.org/obo/GAZ_00068781"/>
        <obo:IAO_0000115>A district of Puriscal Canton.</obo:IAO_0000115>
        <oboInOwl:hasOBONamespace>GAZ</oboInOwl:hasOBONamespace>
        <oboInOwl:id>GAZ:00119231</oboInOwl:id>
        <rdfs:label>San Antonio District</rdfs:label>
    </owl:NamedIndividual>
    


    <!-- http://purl.obolibrary.org/obo/GAZ_00119232 -->

    <owl:NamedIndividual rdf:about="http://purl.obolibrary.org/obo/GAZ_00119232">
        <rdf:type rdf:resource="http://purl.obolibrary.org/obo/ENVO_00000004"/>
        <obo:RO_0001025 rdf:resource="http://purl.obolibrary.org/obo/GAZ_00068781"/>
        <obo:IAO_0000115>A district of Puriscal Canton.</obo:IAO_0000115>
        <oboInOwl:hasOBONamespace>GAZ</oboInOwl:hasOBONamespace>
        <oboInOwl:id>GAZ:00119232</oboInOwl:id>
        <rdfs:label>Grifo Alto District</rdfs:label>
    </owl:NamedIndividual>
    


    <!-- http://purl.obolibrary.org/obo/GAZ_00119233 -->

    <owl:NamedIndividual rdf:about="http://purl.obolibrary.org/obo/GAZ_00119233">
        <rdf:type rdf:resource="http://purl.obolibrary.org/obo/ENVO_00000004"/>
        <obo:RO_0001025 rdf:resource="http://purl.obolibrary.org/obo/GAZ_00068781"/>
        <obo:IAO_0000115>A district of Puriscal Canton.</obo:IAO_0000115>
        <oboInOwl:hasOBONamespace>GAZ</oboInOwl:hasOBONamespace>
        <oboInOwl:id>GAZ:00119233</oboInOwl:id>
        <rdfs:label>Chires District</rdfs:label>
    </owl:NamedIndividual>
    


    <!-- http://purl.obolibrary.org/obo/GAZ_00119234 -->

    <owl:NamedIndividual rdf:about="http://purl.obolibrary.org/obo/GAZ_00119234">
        <rdf:type rdf:resource="http://purl.obolibrary.org/obo/ENVO_00000004"/>
        <obo:RO_0001025 rdf:resource="http://purl.obolibrary.org/obo/GAZ_00068781"/>
        <obo:IAO_0000115>A district of Puriscal Canton.</obo:IAO_0000115>
        <oboInOwl:hasOBONamespace>GAZ</oboInOwl:hasOBONamespace>
        <oboInOwl:id>GAZ:00119234</oboInOwl:id>
        <rdfs:label>Candelarita District</rdfs:label>
    </owl:NamedIndividual>
    


    <!-- http://purl.obolibrary.org/obo/GAZ_00119235 -->

    <owl:NamedIndividual rdf:about="http://purl.obolibrary.org/obo/GAZ_00119235">
        <rdf:type rdf:resource="http://purl.obolibrary.org/obo/ENVO_00000004"/>
        <obo:RO_0001025 rdf:resource="http://purl.obolibrary.org/obo/GAZ_00068781"/>
        <obo:IAO_0000115>A district of Puriscal Canton.</obo:IAO_0000115>
        <oboInOwl:hasOBONamespace>GAZ</oboInOwl:hasOBONamespace>
        <oboInOwl:id>GAZ:00119235</oboInOwl:id>
        <rdfs:label>San Rafael District</rdfs:label>
    </owl:NamedIndividual>
    


    <!-- http://purl.obolibrary.org/obo/GAZ_00119236 -->

    <owl:NamedIndividual rdf:about="http://purl.obolibrary.org/obo/GAZ_00119236">
        <rdf:type rdf:resource="http://purl.obolibrary.org/obo/ENVO_00000004"/>
        <obo:RO_0001025 rdf:resource="http://purl.obolibrary.org/obo/GAZ_00068777"/>
        <obo:IAO_0000115>A district of Tarrazu Canton.</obo:IAO_0000115>
        <oboInOwl:hasOBONamespace>GAZ</oboInOwl:hasOBONamespace>
        <oboInOwl:id>GAZ:00119236</oboInOwl:id>
        <rdfs:label>San Lorenzo District</rdfs:label>
    </owl:NamedIndividual>
    


    <!-- http://purl.obolibrary.org/obo/GAZ_00119237 -->

    <owl:NamedIndividual rdf:about="http://purl.obolibrary.org/obo/GAZ_00119237">
        <obo:RO_0001025 rdf:resource="http://purl.obolibrary.org/obo/GAZ_00068777"/>
        <oboInOwl:hasOBONamespace>GAZ</oboInOwl:hasOBONamespace>
        <oboInOwl:id>GAZ:00119237</oboInOwl:id>
        <rdfs:label>San Marcos District</rdfs:label>
    </owl:NamedIndividual>
    


    <!-- http://purl.obolibrary.org/obo/GAZ_00119238 -->

    <owl:NamedIndividual rdf:about="http://purl.obolibrary.org/obo/GAZ_00119238">
        <rdf:type rdf:resource="http://purl.obolibrary.org/obo/ENVO_00000004"/>
        <obo:RO_0001025 rdf:resource="http://purl.obolibrary.org/obo/GAZ_00068777"/>
        <obo:IAO_0000115>A district of Tarrazu Canton.</obo:IAO_0000115>
        <oboInOwl:hasOBONamespace>GAZ</oboInOwl:hasOBONamespace>
        <oboInOwl:id>GAZ:00119238</oboInOwl:id>
        <rdfs:label>San Carlos District</rdfs:label>
    </owl:NamedIndividual>
    


    <!-- http://purl.obolibrary.org/obo/GAZ_00119239 -->

    <owl:NamedIndividual rdf:about="http://purl.obolibrary.org/obo/GAZ_00119239">
        <rdf:type rdf:resource="http://purl.obolibrary.org/obo/ENVO_00000004"/>
        <obo:RO_0001025 rdf:resource="http://purl.obolibrary.org/obo/GAZ_00068774"/>
        <obo:IAO_0000115>A district of Aserri Canton.</obo:IAO_0000115>
        <oboInOwl:hasOBONamespace>GAZ</oboInOwl:hasOBONamespace>
        <oboInOwl:id>GAZ:00119239</oboInOwl:id>
        <rdfs:label>Tarbaca District</rdfs:label>
    </owl:NamedIndividual>
    


    <!-- http://purl.obolibrary.org/obo/GAZ_00119240 -->

    <owl:NamedIndividual rdf:about="http://purl.obolibrary.org/obo/GAZ_00119240">
        <rdf:type rdf:resource="http://purl.obolibrary.org/obo/ENVO_00000004"/>
        <obo:RO_0001025 rdf:resource="http://purl.obolibrary.org/obo/GAZ_00068774"/>
        <obo:IAO_0000115>A district of Aserri Canton.</obo:IAO_0000115>
        <oboInOwl:hasOBONamespace>GAZ</oboInOwl:hasOBONamespace>
        <oboInOwl:id>GAZ:00119240</oboInOwl:id>
        <rdfs:label>Vuelta de Jorco District</rdfs:label>
    </owl:NamedIndividual>
    


    <!-- http://purl.obolibrary.org/obo/GAZ_00119241 -->

    <owl:NamedIndividual rdf:about="http://purl.obolibrary.org/obo/GAZ_00119241">
        <rdf:type rdf:resource="http://purl.obolibrary.org/obo/ENVO_00000004"/>
        <obo:RO_0001025 rdf:resource="http://purl.obolibrary.org/obo/GAZ_00068774"/>
        <obo:IAO_0000115>A district of Aserri Canton.</obo:IAO_0000115>
        <oboInOwl:hasOBONamespace>GAZ</oboInOwl:hasOBONamespace>
        <oboInOwl:id>GAZ:00119241</oboInOwl:id>
        <rdfs:label>Salitrillos District</rdfs:label>
    </owl:NamedIndividual>
    


    <!-- http://purl.obolibrary.org/obo/GAZ_00119242 -->

    <owl:NamedIndividual rdf:about="http://purl.obolibrary.org/obo/GAZ_00119242">
        <rdf:type rdf:resource="http://purl.obolibrary.org/obo/ENVO_00000004"/>
        <obo:RO_0001025 rdf:resource="http://purl.obolibrary.org/obo/GAZ_00068774"/>
        <obo:IAO_0000115>A district of Aserri Canton.</obo:IAO_0000115>
        <oboInOwl:hasOBONamespace>GAZ</oboInOwl:hasOBONamespace>
        <oboInOwl:id>GAZ:00119242</oboInOwl:id>
        <rdfs:label>San Gabriel District</rdfs:label>
    </owl:NamedIndividual>
    


    <!-- http://purl.obolibrary.org/obo/GAZ_00119243 -->

    <owl:NamedIndividual rdf:about="http://purl.obolibrary.org/obo/GAZ_00119243">
        <rdf:type rdf:resource="http://purl.obolibrary.org/obo/ENVO_00000004"/>
        <obo:RO_0001025 rdf:resource="http://purl.obolibrary.org/obo/GAZ_00068774"/>
        <obo:IAO_0000115>A district of Aserri Canton.</obo:IAO_0000115>
        <oboInOwl:hasOBONamespace>GAZ</oboInOwl:hasOBONamespace>
        <oboInOwl:id>GAZ:00119243</oboInOwl:id>
        <rdfs:label>Monterrey District</rdfs:label>
    </owl:NamedIndividual>
    


    <!-- http://purl.obolibrary.org/obo/GAZ_00119244 -->

    <owl:NamedIndividual rdf:about="http://purl.obolibrary.org/obo/GAZ_00119244">
        <rdf:type rdf:resource="http://purl.obolibrary.org/obo/ENVO_00000004"/>
        <obo:RO_0001025 rdf:resource="http://purl.obolibrary.org/obo/GAZ_00068774"/>
        <obo:IAO_0000115>A district of Aserri Canton.</obo:IAO_0000115>
        <oboInOwl:hasOBONamespace>GAZ</oboInOwl:hasOBONamespace>
        <oboInOwl:id>GAZ:00119244</oboInOwl:id>
        <rdfs:label>La Legua District</rdfs:label>
    </owl:NamedIndividual>
    


    <!-- http://purl.obolibrary.org/obo/GAZ_00119245 -->

    <owl:NamedIndividual rdf:about="http://purl.obolibrary.org/obo/GAZ_00119245">
        <rdf:type rdf:resource="http://purl.obolibrary.org/obo/ENVO_00000004"/>
        <obo:RO_0001025 rdf:resource="http://purl.obolibrary.org/obo/GAZ_00068774"/>
        <obo:IAO_0000115>A district of Aserri Canton.</obo:IAO_0000115>
        <oboInOwl:hasOBONamespace>GAZ</oboInOwl:hasOBONamespace>
        <oboInOwl:id>GAZ:00119245</oboInOwl:id>
        <rdfs:label>Aserri District</rdfs:label>
    </owl:NamedIndividual>
    


    <!-- http://purl.obolibrary.org/obo/GAZ_00119246 -->

    <owl:NamedIndividual rdf:about="http://purl.obolibrary.org/obo/GAZ_00119246">
        <rdf:type rdf:resource="http://purl.obolibrary.org/obo/ENVO_00000004"/>
        <obo:RO_0001025 rdf:resource="http://purl.obolibrary.org/obo/GAZ_00068779"/>
        <obo:IAO_0000115>A district of Mora Canton.</obo:IAO_0000115>
        <oboInOwl:hasOBONamespace>GAZ</oboInOwl:hasOBONamespace>
        <oboInOwl:id>GAZ:00119246</oboInOwl:id>
        <rdfs:label>Colon District</rdfs:label>
    </owl:NamedIndividual>
    


    <!-- http://purl.obolibrary.org/obo/GAZ_00119247 -->

    <owl:NamedIndividual rdf:about="http://purl.obolibrary.org/obo/GAZ_00119247">
        <rdf:type rdf:resource="http://purl.obolibrary.org/obo/ENVO_00000004"/>
        <obo:RO_0001025 rdf:resource="http://purl.obolibrary.org/obo/GAZ_00068779"/>
        <obo:IAO_0000115>A district of Mora Canton.</obo:IAO_0000115>
        <oboInOwl:hasOBONamespace>GAZ</oboInOwl:hasOBONamespace>
        <oboInOwl:id>GAZ:00119247</oboInOwl:id>
        <rdfs:label>Piedras Negras District</rdfs:label>
    </owl:NamedIndividual>
    


    <!-- http://purl.obolibrary.org/obo/GAZ_00119248 -->

    <owl:NamedIndividual rdf:about="http://purl.obolibrary.org/obo/GAZ_00119248">
        <rdf:type rdf:resource="http://purl.obolibrary.org/obo/ENVO_00000004"/>
        <obo:RO_0001025 rdf:resource="http://purl.obolibrary.org/obo/GAZ_00068779"/>
        <obo:IAO_0000115>A district of Mora Canton.</obo:IAO_0000115>
        <oboInOwl:hasOBONamespace>GAZ</oboInOwl:hasOBONamespace>
        <oboInOwl:id>GAZ:00119248</oboInOwl:id>
        <rdfs:label>Picagres District</rdfs:label>
    </owl:NamedIndividual>
    


    <!-- http://purl.obolibrary.org/obo/GAZ_00119249 -->

    <owl:NamedIndividual rdf:about="http://purl.obolibrary.org/obo/GAZ_00119249">
        <rdf:type rdf:resource="http://purl.obolibrary.org/obo/ENVO_00000004"/>
        <obo:RO_0001025 rdf:resource="http://purl.obolibrary.org/obo/GAZ_00068779"/>
        <obo:IAO_0000115>A district of Mora Canton.</obo:IAO_0000115>
        <oboInOwl:hasOBONamespace>GAZ</oboInOwl:hasOBONamespace>
        <oboInOwl:id>GAZ:00119249</oboInOwl:id>
        <rdfs:label>Guayabo District</rdfs:label>
    </owl:NamedIndividual>
    


    <!-- http://purl.obolibrary.org/obo/GAZ_00119250 -->

    <owl:NamedIndividual rdf:about="http://purl.obolibrary.org/obo/GAZ_00119250">
        <rdf:type rdf:resource="http://purl.obolibrary.org/obo/ENVO_00000004"/>
        <obo:RO_0001025 rdf:resource="http://purl.obolibrary.org/obo/GAZ_00068779"/>
        <obo:IAO_0000115>A district of Mora Canton.</obo:IAO_0000115>
        <oboInOwl:hasOBONamespace>GAZ</oboInOwl:hasOBONamespace>
        <oboInOwl:id>GAZ:00119250</oboInOwl:id>
        <rdfs:label>Tabarcia District</rdfs:label>
    </owl:NamedIndividual>
    


    <!-- http://purl.obolibrary.org/obo/GAZ_00119251 -->

    <owl:NamedIndividual rdf:about="http://purl.obolibrary.org/obo/GAZ_00119251">
        <rdf:type rdf:resource="http://purl.obolibrary.org/obo/ENVO_00000004"/>
        <obo:RO_0001025 rdf:resource="http://purl.obolibrary.org/obo/GAZ_00068772"/>
        <obo:IAO_0000115>A district of Goicoechea Canton.</obo:IAO_0000115>
        <oboInOwl:hasOBONamespace>GAZ</oboInOwl:hasOBONamespace>
        <oboInOwl:id>GAZ:00119251</oboInOwl:id>
        <rdfs:label>Mata de Platano District</rdfs:label>
    </owl:NamedIndividual>
    


    <!-- http://purl.obolibrary.org/obo/GAZ_00119252 -->

    <owl:NamedIndividual rdf:about="http://purl.obolibrary.org/obo/GAZ_00119252">
        <rdf:type rdf:resource="http://purl.obolibrary.org/obo/ENVO_00000004"/>
        <obo:RO_0001025 rdf:resource="http://purl.obolibrary.org/obo/GAZ_00068772"/>
        <obo:IAO_0000115>A district of Goicoechea Canton.</obo:IAO_0000115>
        <oboInOwl:hasOBONamespace>GAZ</oboInOwl:hasOBONamespace>
        <oboInOwl:id>GAZ:00119252</oboInOwl:id>
        <rdfs:label>Rancho Redondo District</rdfs:label>
    </owl:NamedIndividual>
    


    <!-- http://purl.obolibrary.org/obo/GAZ_00119253 -->

    <owl:NamedIndividual rdf:about="http://purl.obolibrary.org/obo/GAZ_00119253">
        <rdf:type rdf:resource="http://purl.obolibrary.org/obo/ENVO_00000004"/>
        <obo:RO_0001025 rdf:resource="http://purl.obolibrary.org/obo/GAZ_00068772"/>
        <obo:IAO_0000115>A district of Goicoechea Canton.</obo:IAO_0000115>
        <oboInOwl:hasOBONamespace>GAZ</oboInOwl:hasOBONamespace>
        <oboInOwl:id>GAZ:00119253</oboInOwl:id>
        <rdfs:label>Purral District</rdfs:label>
    </owl:NamedIndividual>
    


    <!-- http://purl.obolibrary.org/obo/GAZ_00119254 -->

    <owl:NamedIndividual rdf:about="http://purl.obolibrary.org/obo/GAZ_00119254">
        <rdf:type rdf:resource="http://purl.obolibrary.org/obo/ENVO_00000004"/>
        <obo:RO_0001025 rdf:resource="http://purl.obolibrary.org/obo/GAZ_00068772"/>
        <obo:IAO_0000115>A district of Goicoechea Canton.</obo:IAO_0000115>
        <oboInOwl:hasOBONamespace>GAZ</oboInOwl:hasOBONamespace>
        <oboInOwl:id>GAZ:00119254</oboInOwl:id>
        <rdfs:label>Guadalupe District</rdfs:label>
    </owl:NamedIndividual>
    


    <!-- http://purl.obolibrary.org/obo/GAZ_00119255 -->

    <owl:NamedIndividual rdf:about="http://purl.obolibrary.org/obo/GAZ_00119255">
        <rdf:type rdf:resource="http://purl.obolibrary.org/obo/ENVO_00000004"/>
        <obo:RO_0001025 rdf:resource="http://purl.obolibrary.org/obo/GAZ_00068772"/>
        <obo:IAO_0000115>A district of Goicoechea Canton.</obo:IAO_0000115>
        <oboInOwl:hasOBONamespace>GAZ</oboInOwl:hasOBONamespace>
        <oboInOwl:id>GAZ:00119255</oboInOwl:id>
        <rdfs:label>Calle Blancos District</rdfs:label>
    </owl:NamedIndividual>
    


    <!-- http://purl.obolibrary.org/obo/GAZ_00119256 -->

    <owl:NamedIndividual rdf:about="http://purl.obolibrary.org/obo/GAZ_00119256">
        <rdf:type rdf:resource="http://purl.obolibrary.org/obo/ENVO_00000004"/>
        <obo:RO_0001025 rdf:resource="http://purl.obolibrary.org/obo/GAZ_00068772"/>
        <obo:IAO_0000115>A district of Goicoechea Canton.</obo:IAO_0000115>
        <oboInOwl:hasOBONamespace>GAZ</oboInOwl:hasOBONamespace>
        <oboInOwl:id>GAZ:00119256</oboInOwl:id>
        <rdfs:label>San Francisco District</rdfs:label>
    </owl:NamedIndividual>
    


    <!-- http://purl.obolibrary.org/obo/GAZ_00119257 -->

    <owl:NamedIndividual rdf:about="http://purl.obolibrary.org/obo/GAZ_00119257">
        <rdf:type rdf:resource="http://purl.obolibrary.org/obo/ENVO_00000004"/>
        <obo:RO_0001025 rdf:resource="http://purl.obolibrary.org/obo/GAZ_00068772"/>
        <obo:IAO_0000115>A district of Goicoechea Canton.</obo:IAO_0000115>
        <oboInOwl:hasOBONamespace>GAZ</oboInOwl:hasOBONamespace>
        <oboInOwl:id>GAZ:00119257</oboInOwl:id>
        <rdfs:label>Ipis District</rdfs:label>
    </owl:NamedIndividual>
    


    <!-- http://purl.obolibrary.org/obo/GAZ_00119258 -->

    <owl:NamedIndividual rdf:about="http://purl.obolibrary.org/obo/GAZ_00119258">
        <rdf:type rdf:resource="http://purl.obolibrary.org/obo/ENVO_00000004"/>
        <obo:RO_0001025 rdf:resource="http://purl.obolibrary.org/obo/GAZ_00068767"/>
        <obo:IAO_0000115>A district of Santa Ana Canton.</obo:IAO_0000115>
        <oboInOwl:hasOBONamespace>GAZ</oboInOwl:hasOBONamespace>
        <oboInOwl:id>GAZ:00119258</oboInOwl:id>
        <rdfs:label>Brasil District</rdfs:label>
    </owl:NamedIndividual>
    


    <!-- http://purl.obolibrary.org/obo/GAZ_00119259 -->

    <owl:NamedIndividual rdf:about="http://purl.obolibrary.org/obo/GAZ_00119259">
        <rdf:type rdf:resource="http://purl.obolibrary.org/obo/ENVO_00000004"/>
        <obo:RO_0001025 rdf:resource="http://purl.obolibrary.org/obo/GAZ_00068767"/>
        <obo:IAO_0000115>A district of Santa Ana Canton.</obo:IAO_0000115>
        <oboInOwl:hasOBONamespace>GAZ</oboInOwl:hasOBONamespace>
        <oboInOwl:id>GAZ:00119259</oboInOwl:id>
        <rdfs:label>Pozos District</rdfs:label>
    </owl:NamedIndividual>
    


    <!-- http://purl.obolibrary.org/obo/GAZ_00119261 -->

    <owl:NamedIndividual rdf:about="http://purl.obolibrary.org/obo/GAZ_00119261">
        <rdf:type rdf:resource="http://purl.obolibrary.org/obo/ENVO_00000004"/>
        <obo:RO_0001025 rdf:resource="http://purl.obolibrary.org/obo/GAZ_00068767"/>
        <obo:IAO_0000115>A district of Santa Ana Canton.</obo:IAO_0000115>
        <oboInOwl:hasOBONamespace>GAZ</oboInOwl:hasOBONamespace>
        <oboInOwl:id>GAZ:00119261</oboInOwl:id>
        <rdfs:label>Uruca District</rdfs:label>
    </owl:NamedIndividual>
    


    <!-- http://purl.obolibrary.org/obo/GAZ_00119262 -->

    <owl:NamedIndividual rdf:about="http://purl.obolibrary.org/obo/GAZ_00119262">
        <rdf:type rdf:resource="http://purl.obolibrary.org/obo/ENVO_00000004"/>
        <obo:RO_0001025 rdf:resource="http://purl.obolibrary.org/obo/GAZ_00068767"/>
        <obo:IAO_0000115>A district of Santa Ana Canton.</obo:IAO_0000115>
        <oboInOwl:hasOBONamespace>GAZ</oboInOwl:hasOBONamespace>
        <oboInOwl:id>GAZ:00119262</oboInOwl:id>
        <rdfs:label>Santa Ana District</rdfs:label>
    </owl:NamedIndividual>
    


    <!-- http://purl.obolibrary.org/obo/GAZ_00119263 -->

    <owl:NamedIndividual rdf:about="http://purl.obolibrary.org/obo/GAZ_00119263">
        <rdf:type rdf:resource="http://purl.obolibrary.org/obo/ENVO_00000004"/>
        <obo:RO_0001025 rdf:resource="http://purl.obolibrary.org/obo/GAZ_00068767"/>
        <obo:IAO_0000115>A district of Santa Ana Canton.</obo:IAO_0000115>
        <oboInOwl:hasOBONamespace>GAZ</oboInOwl:hasOBONamespace>
        <oboInOwl:id>GAZ:00119263</oboInOwl:id>
        <rdfs:label>Piedades District</rdfs:label>
    </owl:NamedIndividual>
    


    <!-- http://purl.obolibrary.org/obo/GAZ_00119264 -->

    <owl:NamedIndividual rdf:about="http://purl.obolibrary.org/obo/GAZ_00119264">
        <rdf:type rdf:resource="http://purl.obolibrary.org/obo/ENVO_00000004"/>
        <obo:RO_0001025 rdf:resource="http://purl.obolibrary.org/obo/GAZ_00068767"/>
        <obo:IAO_0000115>A district of Santa Ana Canton.</obo:IAO_0000115>
        <oboInOwl:hasOBONamespace>GAZ</oboInOwl:hasOBONamespace>
        <oboInOwl:id>GAZ:00119264</oboInOwl:id>
        <rdfs:label>Salitral District</rdfs:label>
    </owl:NamedIndividual>
    


    <!-- http://purl.obolibrary.org/obo/GAZ_00119265 -->

    <owl:NamedIndividual rdf:about="http://purl.obolibrary.org/obo/GAZ_00119265">
        <rdf:type rdf:resource="http://purl.obolibrary.org/obo/ENVO_00000004"/>
        <obo:RO_0001025 rdf:resource="http://purl.obolibrary.org/obo/GAZ_00068783"/>
        <obo:IAO_0000115>A district of Alajuelita Canton.</obo:IAO_0000115>
        <oboInOwl:hasOBONamespace>GAZ</oboInOwl:hasOBONamespace>
        <oboInOwl:id>GAZ:00119265</oboInOwl:id>
        <rdfs:label>San Felipe District</rdfs:label>
    </owl:NamedIndividual>
    


    <!-- http://purl.obolibrary.org/obo/GAZ_00119266 -->

    <owl:NamedIndividual rdf:about="http://purl.obolibrary.org/obo/GAZ_00119266">
        <rdf:type rdf:resource="http://purl.obolibrary.org/obo/ENVO_00000004"/>
        <obo:RO_0001025 rdf:resource="http://purl.obolibrary.org/obo/GAZ_00068783"/>
        <obo:IAO_0000115>A district of Alajuelita Canton.</obo:IAO_0000115>
        <oboInOwl:hasOBONamespace>GAZ</oboInOwl:hasOBONamespace>
        <oboInOwl:id>GAZ:00119266</oboInOwl:id>
        <rdfs:label>Concepcion District</rdfs:label>
    </owl:NamedIndividual>
    


    <!-- http://purl.obolibrary.org/obo/GAZ_00119267 -->

    <owl:NamedIndividual rdf:about="http://purl.obolibrary.org/obo/GAZ_00119267">
        <rdf:type rdf:resource="http://purl.obolibrary.org/obo/ENVO_00000004"/>
        <obo:RO_0001025 rdf:resource="http://purl.obolibrary.org/obo/GAZ_00068783"/>
        <obo:IAO_0000115>A district of Alajuelita Canton.</obo:IAO_0000115>
        <oboInOwl:hasOBONamespace>GAZ</oboInOwl:hasOBONamespace>
        <oboInOwl:id>GAZ:00119267</oboInOwl:id>
        <rdfs:label>San Josecito District</rdfs:label>
    </owl:NamedIndividual>
    


    <!-- http://purl.obolibrary.org/obo/GAZ_00119268 -->

    <owl:NamedIndividual rdf:about="http://purl.obolibrary.org/obo/GAZ_00119268">
        <rdf:type rdf:resource="http://purl.obolibrary.org/obo/ENVO_00000004"/>
        <obo:RO_0001025 rdf:resource="http://purl.obolibrary.org/obo/GAZ_00068783"/>
        <obo:IAO_0000115>A district of Alajuelita Canton.</obo:IAO_0000115>
        <oboInOwl:hasOBONamespace>GAZ</oboInOwl:hasOBONamespace>
        <oboInOwl:id>GAZ:00119268</oboInOwl:id>
        <rdfs:label>San Antonio District</rdfs:label>
    </owl:NamedIndividual>
    


    <!-- http://purl.obolibrary.org/obo/GAZ_00119269 -->

    <owl:NamedIndividual rdf:about="http://purl.obolibrary.org/obo/GAZ_00119269">
        <rdf:type rdf:resource="http://purl.obolibrary.org/obo/ENVO_00000004"/>
        <obo:RO_0001025 rdf:resource="http://purl.obolibrary.org/obo/GAZ_00068783"/>
        <obo:IAO_0000115>A district of Alajuelita Canton.</obo:IAO_0000115>
        <oboInOwl:hasOBONamespace>GAZ</oboInOwl:hasOBONamespace>
        <oboInOwl:id>GAZ:00119269</oboInOwl:id>
        <rdfs:label>Alajuelita District</rdfs:label>
    </owl:NamedIndividual>
    


    <!-- http://purl.obolibrary.org/obo/GAZ_00119270 -->

    <owl:NamedIndividual rdf:about="http://purl.obolibrary.org/obo/GAZ_00119270">
        <rdf:type rdf:resource="http://purl.obolibrary.org/obo/ENVO_00000004"/>
        <obo:RO_0001025 rdf:resource="http://purl.obolibrary.org/obo/GAZ_00068773"/>
        <obo:IAO_0000115>A district of Vasquez de Coronado Canton.</obo:IAO_0000115>
        <oboInOwl:hasOBONamespace>GAZ</oboInOwl:hasOBONamespace>
        <oboInOwl:id>GAZ:00119270</oboInOwl:id>
        <rdfs:label>Patalillo District</rdfs:label>
    </owl:NamedIndividual>
    


    <!-- http://purl.obolibrary.org/obo/GAZ_00119271 -->

    <owl:NamedIndividual rdf:about="http://purl.obolibrary.org/obo/GAZ_00119271">
        <rdf:type rdf:resource="http://purl.obolibrary.org/obo/ENVO_00000004"/>
        <obo:RO_0001025 rdf:resource="http://purl.obolibrary.org/obo/GAZ_00068773"/>
        <obo:IAO_0000115>A district of Vasquez de Coronado Canton.</obo:IAO_0000115>
        <oboInOwl:hasOBONamespace>GAZ</oboInOwl:hasOBONamespace>
        <oboInOwl:id>GAZ:00119271</oboInOwl:id>
        <rdfs:label>San Rafael District</rdfs:label>
    </owl:NamedIndividual>
    


    <!-- http://purl.obolibrary.org/obo/GAZ_00119272 -->

    <owl:NamedIndividual rdf:about="http://purl.obolibrary.org/obo/GAZ_00119272">
        <rdf:type rdf:resource="http://purl.obolibrary.org/obo/ENVO_00000004"/>
        <obo:RO_0001025 rdf:resource="http://purl.obolibrary.org/obo/GAZ_00068773"/>
        <obo:IAO_0000115>A district of Vasquez de Coronado Canton.</obo:IAO_0000115>
        <oboInOwl:hasOBONamespace>GAZ</oboInOwl:hasOBONamespace>
        <oboInOwl:id>GAZ:00119272</oboInOwl:id>
        <rdfs:label>Dulce Nombre de Jesus District</rdfs:label>
    </owl:NamedIndividual>
    


    <!-- http://purl.obolibrary.org/obo/GAZ_00119273 -->

    <owl:NamedIndividual rdf:about="http://purl.obolibrary.org/obo/GAZ_00119273">
        <rdf:type rdf:resource="http://purl.obolibrary.org/obo/ENVO_00000004"/>
        <obo:RO_0001025 rdf:resource="http://purl.obolibrary.org/obo/GAZ_00068773"/>
        <obo:IAO_0000115>A district of Vasquez de Coronado Canton.</obo:IAO_0000115>
        <oboInOwl:hasOBONamespace>GAZ</oboInOwl:hasOBONamespace>
        <oboInOwl:id>GAZ:00119273</oboInOwl:id>
        <rdfs:label>San Isidro District</rdfs:label>
    </owl:NamedIndividual>
    


    <!-- http://purl.obolibrary.org/obo/GAZ_00119274 -->

    <owl:NamedIndividual rdf:about="http://purl.obolibrary.org/obo/GAZ_00119274">
        <rdf:type rdf:resource="http://purl.obolibrary.org/obo/ENVO_00000004"/>
        <obo:RO_0001025 rdf:resource="http://purl.obolibrary.org/obo/GAZ_00068773"/>
        <obo:IAO_0000115>A district of Vasquez de Coronado Canton.</obo:IAO_0000115>
        <oboInOwl:hasOBONamespace>GAZ</oboInOwl:hasOBONamespace>
        <oboInOwl:id>GAZ:00119274</oboInOwl:id>
        <rdfs:label>Cascajal District</rdfs:label>
    </owl:NamedIndividual>
    


    <!-- http://purl.obolibrary.org/obo/GAZ_00119275 -->

    <owl:NamedIndividual rdf:about="http://purl.obolibrary.org/obo/GAZ_00119275">
        <rdf:type rdf:resource="http://purl.obolibrary.org/obo/ENVO_00000004"/>
        <obo:RO_0001025 rdf:resource="http://purl.obolibrary.org/obo/GAZ_00068782"/>
        <obo:IAO_0000115>A district of Acosta Canton.</obo:IAO_0000115>
        <oboInOwl:hasOBONamespace>GAZ</oboInOwl:hasOBONamespace>
        <oboInOwl:id>GAZ:00119275</oboInOwl:id>
        <rdfs:label>Cangrejal District</rdfs:label>
    </owl:NamedIndividual>
    


    <!-- http://purl.obolibrary.org/obo/GAZ_00119276 -->

    <owl:NamedIndividual rdf:about="http://purl.obolibrary.org/obo/GAZ_00119276">
        <rdf:type rdf:resource="http://purl.obolibrary.org/obo/ENVO_00000004"/>
        <obo:RO_0001025 rdf:resource="http://purl.obolibrary.org/obo/GAZ_00068782"/>
        <obo:IAO_0000115>A district of Acosta Canton.</obo:IAO_0000115>
        <oboInOwl:hasOBONamespace>GAZ</oboInOwl:hasOBONamespace>
        <oboInOwl:id>GAZ:00119276</oboInOwl:id>
        <rdfs:label>Guaitil District</rdfs:label>
    </owl:NamedIndividual>
    


    <!-- http://purl.obolibrary.org/obo/GAZ_00119277 -->

    <owl:NamedIndividual rdf:about="http://purl.obolibrary.org/obo/GAZ_00119277">
        <rdf:type rdf:resource="http://purl.obolibrary.org/obo/ENVO_00000004"/>
        <obo:RO_0001025 rdf:resource="http://purl.obolibrary.org/obo/GAZ_00068782"/>
        <obo:IAO_0000115>A district of Acosta Canton.</obo:IAO_0000115>
        <oboInOwl:hasOBONamespace>GAZ</oboInOwl:hasOBONamespace>
        <oboInOwl:id>GAZ:00119277</oboInOwl:id>
        <rdfs:label>Sabanillas District</rdfs:label>
    </owl:NamedIndividual>
    


    <!-- http://purl.obolibrary.org/obo/GAZ_00119278 -->

    <owl:NamedIndividual rdf:about="http://purl.obolibrary.org/obo/GAZ_00119278">
        <rdf:type rdf:resource="http://purl.obolibrary.org/obo/ENVO_00000004"/>
        <obo:RO_0001025 rdf:resource="http://purl.obolibrary.org/obo/GAZ_00068782"/>
        <obo:IAO_0000115>A district of Acosta Canton.</obo:IAO_0000115>
        <oboInOwl:hasOBONamespace>GAZ</oboInOwl:hasOBONamespace>
        <oboInOwl:id>GAZ:00119278</oboInOwl:id>
        <rdfs:label>San Ignacio District</rdfs:label>
    </owl:NamedIndividual>
    


    <!-- http://purl.obolibrary.org/obo/GAZ_00119279 -->

    <owl:NamedIndividual rdf:about="http://purl.obolibrary.org/obo/GAZ_00119279">
        <rdf:type rdf:resource="http://purl.obolibrary.org/obo/ENVO_00000004"/>
        <obo:RO_0001025 rdf:resource="http://purl.obolibrary.org/obo/GAZ_00068782"/>
        <obo:IAO_0000115>A district of Acosta Canton.</obo:IAO_0000115>
        <oboInOwl:hasOBONamespace>GAZ</oboInOwl:hasOBONamespace>
        <oboInOwl:id>GAZ:00119279</oboInOwl:id>
        <rdfs:label>Palmichal District</rdfs:label>
    </owl:NamedIndividual>
    


    <!-- http://purl.obolibrary.org/obo/GAZ_00119280 -->

    <owl:NamedIndividual rdf:about="http://purl.obolibrary.org/obo/GAZ_00119280">
        <rdf:type rdf:resource="http://purl.obolibrary.org/obo/ENVO_00000004"/>
        <obo:RO_0001025 rdf:resource="http://purl.obolibrary.org/obo/GAZ_00068769"/>
        <obo:IAO_0000115>A district of Tibas Canton.</obo:IAO_0000115>
        <oboInOwl:hasOBONamespace>GAZ</oboInOwl:hasOBONamespace>
        <oboInOwl:id>GAZ:00119280</oboInOwl:id>
        <rdfs:label>San Juan District</rdfs:label>
    </owl:NamedIndividual>
    


    <!-- http://purl.obolibrary.org/obo/GAZ_00119281 -->

    <owl:NamedIndividual rdf:about="http://purl.obolibrary.org/obo/GAZ_00119281">
        <rdf:type rdf:resource="http://purl.obolibrary.org/obo/ENVO_00000004"/>
        <obo:RO_0001025 rdf:resource="http://purl.obolibrary.org/obo/GAZ_00068769"/>
        <obo:IAO_0000115>A district of Tibas Canton.</obo:IAO_0000115>
        <oboInOwl:hasOBONamespace>GAZ</oboInOwl:hasOBONamespace>
        <oboInOwl:id>GAZ:00119281</oboInOwl:id>
        <rdfs:label>Cinco Esquinas District</rdfs:label>
    </owl:NamedIndividual>
    


    <!-- http://purl.obolibrary.org/obo/GAZ_00119282 -->

    <owl:NamedIndividual rdf:about="http://purl.obolibrary.org/obo/GAZ_00119282">
        <rdf:type rdf:resource="http://purl.obolibrary.org/obo/ENVO_00000004"/>
        <obo:RO_0001025 rdf:resource="http://purl.obolibrary.org/obo/GAZ_00068769"/>
        <obo:IAO_0000115>A district of Tibas Canton.</obo:IAO_0000115>
        <oboInOwl:hasOBONamespace>GAZ</oboInOwl:hasOBONamespace>
        <oboInOwl:id>GAZ:00119282</oboInOwl:id>
        <rdfs:label>Leon XIII District</rdfs:label>
    </owl:NamedIndividual>
    


    <!-- http://purl.obolibrary.org/obo/GAZ_00119283 -->

    <owl:NamedIndividual rdf:about="http://purl.obolibrary.org/obo/GAZ_00119283">
        <rdf:type rdf:resource="http://purl.obolibrary.org/obo/ENVO_00000004"/>
        <obo:RO_0001025 rdf:resource="http://purl.obolibrary.org/obo/GAZ_00068769"/>
        <obo:IAO_0000115>A district of Tibas Canton.</obo:IAO_0000115>
        <oboInOwl:hasOBONamespace>GAZ</oboInOwl:hasOBONamespace>
        <oboInOwl:id>GAZ:00119283</oboInOwl:id>
        <rdfs:label>Colim District</rdfs:label>
    </owl:NamedIndividual>
    


    <!-- http://purl.obolibrary.org/obo/GAZ_00119284 -->

    <owl:NamedIndividual rdf:about="http://purl.obolibrary.org/obo/GAZ_00119284">
        <rdf:type rdf:resource="http://purl.obolibrary.org/obo/ENVO_00000004"/>
        <obo:RO_0001025 rdf:resource="http://purl.obolibrary.org/obo/GAZ_00068769"/>
        <obo:IAO_0000115>A district of Tibas Canton.</obo:IAO_0000115>
        <oboInOwl:hasOBONamespace>GAZ</oboInOwl:hasOBONamespace>
        <oboInOwl:id>GAZ:00119284</oboInOwl:id>
        <rdfs:label>Anselmo Llorente District</rdfs:label>
    </owl:NamedIndividual>
    


    <!-- http://purl.obolibrary.org/obo/GAZ_00119285 -->

    <owl:NamedIndividual rdf:about="http://purl.obolibrary.org/obo/GAZ_00119285">
        <rdf:type rdf:resource="http://purl.obolibrary.org/obo/ENVO_00000004"/>
        <obo:RO_0001025 rdf:resource="http://purl.obolibrary.org/obo/GAZ_00068771"/>
        <obo:IAO_0000115>A district of Moravia Canton.</obo:IAO_0000115>
        <oboInOwl:hasOBONamespace>GAZ</oboInOwl:hasOBONamespace>
        <oboInOwl:id>GAZ:00119285</oboInOwl:id>
        <rdfs:label>San Jeronimo District</rdfs:label>
    </owl:NamedIndividual>
    


    <!-- http://purl.obolibrary.org/obo/GAZ_00119286 -->

    <owl:NamedIndividual rdf:about="http://purl.obolibrary.org/obo/GAZ_00119286">
        <rdf:type rdf:resource="http://purl.obolibrary.org/obo/ENVO_00000004"/>
        <obo:RO_0001025 rdf:resource="http://purl.obolibrary.org/obo/GAZ_00068771"/>
        <obo:IAO_0000115>A district of Moravia Canton.</obo:IAO_0000115>
        <oboInOwl:hasOBONamespace>GAZ</oboInOwl:hasOBONamespace>
        <oboInOwl:id>GAZ:00119286</oboInOwl:id>
        <rdfs:label>San Vincente District</rdfs:label>
    </owl:NamedIndividual>
    


    <!-- http://purl.obolibrary.org/obo/GAZ_00119287 -->

    <owl:NamedIndividual rdf:about="http://purl.obolibrary.org/obo/GAZ_00119287">
        <rdf:type rdf:resource="http://purl.obolibrary.org/obo/ENVO_00000004"/>
        <obo:RO_0001025 rdf:resource="http://purl.obolibrary.org/obo/GAZ_00068771"/>
        <obo:IAO_0000115>A district of Moravia Canton.</obo:IAO_0000115>
        <oboInOwl:hasOBONamespace>GAZ</oboInOwl:hasOBONamespace>
        <oboInOwl:id>GAZ:00119287</oboInOwl:id>
        <rdfs:label>La Trinidad District</rdfs:label>
    </owl:NamedIndividual>
    


    <!-- http://purl.obolibrary.org/obo/GAZ_00119288 -->

    <owl:NamedIndividual rdf:about="http://purl.obolibrary.org/obo/GAZ_00119288">
        <rdf:type rdf:resource="http://purl.obolibrary.org/obo/ENVO_00000004"/>
        <obo:RO_0001025 rdf:resource="http://purl.obolibrary.org/obo/GAZ_00068780"/>
        <obo:IAO_0000115>A district in Montes de Oca Canton.</obo:IAO_0000115>
        <oboInOwl:hasOBONamespace>GAZ</oboInOwl:hasOBONamespace>
        <oboInOwl:id>GAZ:00119288</oboInOwl:id>
        <rdfs:label>San Rafael District</rdfs:label>
    </owl:NamedIndividual>
    


    <!-- http://purl.obolibrary.org/obo/GAZ_00119289 -->

    <owl:NamedIndividual rdf:about="http://purl.obolibrary.org/obo/GAZ_00119289">
        <rdf:type rdf:resource="http://purl.obolibrary.org/obo/ENVO_00000004"/>
        <obo:RO_0001025 rdf:resource="http://purl.obolibrary.org/obo/GAZ_00068780"/>
        <obo:IAO_0000115>A district in Montes de Oca Canton.</obo:IAO_0000115>
        <oboInOwl:hasOBONamespace>GAZ</oboInOwl:hasOBONamespace>
        <oboInOwl:id>GAZ:00119289</oboInOwl:id>
        <rdfs:label>Mercedes District</rdfs:label>
    </owl:NamedIndividual>
    


    <!-- http://purl.obolibrary.org/obo/GAZ_00119290 -->

    <owl:NamedIndividual rdf:about="http://purl.obolibrary.org/obo/GAZ_00119290">
        <rdf:type rdf:resource="http://purl.obolibrary.org/obo/ENVO_00000004"/>
        <obo:RO_0001025 rdf:resource="http://purl.obolibrary.org/obo/GAZ_00068780"/>
        <obo:IAO_0000115>A district in Montes de Oca Canton.</obo:IAO_0000115>
        <oboInOwl:hasOBONamespace>GAZ</oboInOwl:hasOBONamespace>
        <oboInOwl:id>GAZ:00119290</oboInOwl:id>
        <rdfs:label>Sabanilla District</rdfs:label>
    </owl:NamedIndividual>
    


    <!-- http://purl.obolibrary.org/obo/GAZ_00119291 -->

    <owl:NamedIndividual rdf:about="http://purl.obolibrary.org/obo/GAZ_00119291">
        <rdf:type rdf:resource="http://purl.obolibrary.org/obo/ENVO_00000004"/>
        <obo:RO_0001025 rdf:resource="http://purl.obolibrary.org/obo/GAZ_00068780"/>
        <obo:IAO_0000115>A district in Montes de Oca Canton.</obo:IAO_0000115>
        <oboInOwl:hasOBONamespace>GAZ</oboInOwl:hasOBONamespace>
        <oboInOwl:id>GAZ:00119291</oboInOwl:id>
        <rdfs:label>San Pedro District</rdfs:label>
    </owl:NamedIndividual>
    


    <!-- http://purl.obolibrary.org/obo/GAZ_00119292 -->

    <owl:NamedIndividual rdf:about="http://purl.obolibrary.org/obo/GAZ_00119292">
        <rdf:type rdf:resource="http://purl.obolibrary.org/obo/ENVO_00000004"/>
        <obo:RO_0001025 rdf:resource="http://purl.obolibrary.org/obo/GAZ_00068775"/>
        <obo:IAO_0000115>A district in Turrubares Canton.</obo:IAO_0000115>
        <oboInOwl:hasOBONamespace>GAZ</oboInOwl:hasOBONamespace>
        <oboInOwl:id>GAZ:00119292</oboInOwl:id>
        <rdfs:label>San Pablo District</rdfs:label>
    </owl:NamedIndividual>
    


    <!-- http://purl.obolibrary.org/obo/GAZ_00119293 -->

    <owl:NamedIndividual rdf:about="http://purl.obolibrary.org/obo/GAZ_00119293">
        <rdf:type rdf:resource="http://purl.obolibrary.org/obo/ENVO_00000004"/>
        <obo:RO_0001025 rdf:resource="http://purl.obolibrary.org/obo/GAZ_00068775"/>
        <obo:IAO_0000115>A district in Turrubares Canton.</obo:IAO_0000115>
        <oboInOwl:hasOBONamespace>GAZ</oboInOwl:hasOBONamespace>
        <oboInOwl:id>GAZ:00119293</oboInOwl:id>
        <rdfs:label>San Juan de Mata District</rdfs:label>
    </owl:NamedIndividual>
    


    <!-- http://purl.obolibrary.org/obo/GAZ_00119294 -->

    <owl:NamedIndividual rdf:about="http://purl.obolibrary.org/obo/GAZ_00119294">
        <rdf:type rdf:resource="http://purl.obolibrary.org/obo/ENVO_00000004"/>
        <obo:RO_0001025 rdf:resource="http://purl.obolibrary.org/obo/GAZ_00068775"/>
        <obo:IAO_0000115>A district in Turrubares Canton.</obo:IAO_0000115>
        <oboInOwl:hasOBONamespace>GAZ</oboInOwl:hasOBONamespace>
        <oboInOwl:id>GAZ:00119294</oboInOwl:id>
        <rdfs:label>San Pedro District</rdfs:label>
    </owl:NamedIndividual>
    


    <!-- http://purl.obolibrary.org/obo/GAZ_00119295 -->

    <owl:NamedIndividual rdf:about="http://purl.obolibrary.org/obo/GAZ_00119295">
        <rdf:type rdf:resource="http://purl.obolibrary.org/obo/ENVO_00000004"/>
        <obo:RO_0001025 rdf:resource="http://purl.obolibrary.org/obo/GAZ_00068775"/>
        <obo:IAO_0000115>A district in Turrubares Canton.</obo:IAO_0000115>
        <oboInOwl:hasOBONamespace>GAZ</oboInOwl:hasOBONamespace>
        <oboInOwl:id>GAZ:00119295</oboInOwl:id>
        <rdfs:label>San Luis District</rdfs:label>
    </owl:NamedIndividual>
    


    <!-- http://purl.obolibrary.org/obo/GAZ_00119297 -->

    <owl:NamedIndividual rdf:about="http://purl.obolibrary.org/obo/GAZ_00119297">
        <rdf:type rdf:resource="http://purl.obolibrary.org/obo/ENVO_00000004"/>
        <obo:RO_0001025 rdf:resource="http://purl.obolibrary.org/obo/GAZ_00068778"/>
        <obo:IAO_0000115>A district of Dota Canton.</obo:IAO_0000115>
        <oboInOwl:hasOBONamespace>GAZ</oboInOwl:hasOBONamespace>
        <oboInOwl:id>GAZ:00119297</oboInOwl:id>
        <rdfs:label>Santa Maria District</rdfs:label>
    </owl:NamedIndividual>
    


    <!-- http://purl.obolibrary.org/obo/GAZ_00119298 -->

    <owl:NamedIndividual rdf:about="http://purl.obolibrary.org/obo/GAZ_00119298">
        <rdf:type rdf:resource="http://purl.obolibrary.org/obo/ENVO_00000004"/>
        <obo:RO_0001025 rdf:resource="http://purl.obolibrary.org/obo/GAZ_00068778"/>
        <obo:IAO_0000115>A district of Dota Canton.</obo:IAO_0000115>
        <oboInOwl:hasOBONamespace>GAZ</oboInOwl:hasOBONamespace>
        <oboInOwl:id>GAZ:00119298</oboInOwl:id>
        <rdfs:label>Jardin District</rdfs:label>
    </owl:NamedIndividual>
    


    <!-- http://purl.obolibrary.org/obo/GAZ_00119299 -->

    <owl:NamedIndividual rdf:about="http://purl.obolibrary.org/obo/GAZ_00119299">
        <rdf:type rdf:resource="http://purl.obolibrary.org/obo/ENVO_00000004"/>
        <obo:RO_0001025 rdf:resource="http://purl.obolibrary.org/obo/GAZ_00068778"/>
        <obo:IAO_0000115>A district of Dota Canton.</obo:IAO_0000115>
        <oboInOwl:hasOBONamespace>GAZ</oboInOwl:hasOBONamespace>
        <oboInOwl:id>GAZ:00119299</oboInOwl:id>
        <rdfs:label>Copey District</rdfs:label>
    </owl:NamedIndividual>
    


    <!-- http://purl.obolibrary.org/obo/GAZ_00119300 -->

    <owl:NamedIndividual rdf:about="http://purl.obolibrary.org/obo/GAZ_00119300">
        <rdf:type rdf:resource="http://purl.obolibrary.org/obo/ENVO_00000004"/>
        <obo:RO_0001025 rdf:resource="http://purl.obolibrary.org/obo/GAZ_00068770"/>
        <obo:IAO_0000115>A district of Curridabat Canton.</obo:IAO_0000115>
        <oboInOwl:hasOBONamespace>GAZ</oboInOwl:hasOBONamespace>
        <oboInOwl:id>GAZ:00119300</oboInOwl:id>
        <rdfs:label>Granadilla District</rdfs:label>
    </owl:NamedIndividual>
    


    <!-- http://purl.obolibrary.org/obo/GAZ_00119301 -->

    <owl:NamedIndividual rdf:about="http://purl.obolibrary.org/obo/GAZ_00119301">
        <rdf:type rdf:resource="http://purl.obolibrary.org/obo/ENVO_00000004"/>
        <obo:RO_0001025 rdf:resource="http://purl.obolibrary.org/obo/GAZ_00068770"/>
        <obo:IAO_0000115>A district of Curridabat Canton.</obo:IAO_0000115>
        <oboInOwl:hasOBONamespace>GAZ</oboInOwl:hasOBONamespace>
        <oboInOwl:id>GAZ:00119301</oboInOwl:id>
        <rdfs:label>Sanchez District</rdfs:label>
    </owl:NamedIndividual>
    


    <!-- http://purl.obolibrary.org/obo/GAZ_00119302 -->

    <owl:NamedIndividual rdf:about="http://purl.obolibrary.org/obo/GAZ_00119302">
        <rdf:type rdf:resource="http://purl.obolibrary.org/obo/ENVO_00000004"/>
        <obo:RO_0001025 rdf:resource="http://purl.obolibrary.org/obo/GAZ_00068770"/>
        <obo:IAO_0000115>A district of Curridabat Canton.</obo:IAO_0000115>
        <oboInOwl:hasOBONamespace>GAZ</oboInOwl:hasOBONamespace>
        <oboInOwl:id>GAZ:00119302</oboInOwl:id>
        <rdfs:label>Tirrases District</rdfs:label>
    </owl:NamedIndividual>
    


    <!-- http://purl.obolibrary.org/obo/GAZ_00119303 -->

    <owl:NamedIndividual rdf:about="http://purl.obolibrary.org/obo/GAZ_00119303">
        <rdf:type rdf:resource="http://purl.obolibrary.org/obo/ENVO_00000004"/>
        <obo:RO_0001025 rdf:resource="http://purl.obolibrary.org/obo/GAZ_00068770"/>
        <obo:IAO_0000115>A district of Curridabat Canton.</obo:IAO_0000115>
        <oboInOwl:hasOBONamespace>GAZ</oboInOwl:hasOBONamespace>
        <oboInOwl:id>GAZ:00119303</oboInOwl:id>
        <rdfs:label>Curridabat District</rdfs:label>
    </owl:NamedIndividual>
    


    <!-- http://purl.obolibrary.org/obo/GAZ_00119304 -->

    <owl:NamedIndividual rdf:about="http://purl.obolibrary.org/obo/GAZ_00119304">
        <rdf:type rdf:resource="http://purl.obolibrary.org/obo/ENVO_00000004"/>
        <obo:RO_0001025 rdf:resource="http://purl.obolibrary.org/obo/GAZ_00068776"/>
        <obo:IAO_0000115>A district in Perez Zeledon Canton.</obo:IAO_0000115>
        <oboInOwl:hasOBONamespace>GAZ</oboInOwl:hasOBONamespace>
        <oboInOwl:id>GAZ:00119304</oboInOwl:id>
        <rdfs:label>Pejibaye District</rdfs:label>
    </owl:NamedIndividual>
    


    <!-- http://purl.obolibrary.org/obo/GAZ_00119305 -->

    <owl:NamedIndividual rdf:about="http://purl.obolibrary.org/obo/GAZ_00119305">
        <rdf:type rdf:resource="http://purl.obolibrary.org/obo/ENVO_00000004"/>
        <obo:RO_0001025 rdf:resource="http://purl.obolibrary.org/obo/GAZ_00068776"/>
        <obo:IAO_0000115>A district in Perez Zeledon Canton.</obo:IAO_0000115>
        <oboInOwl:hasOBONamespace>GAZ</oboInOwl:hasOBONamespace>
        <oboInOwl:id>GAZ:00119305</oboInOwl:id>
        <rdfs:label>Daniel Flores District</rdfs:label>
    </owl:NamedIndividual>
    


    <!-- http://purl.obolibrary.org/obo/GAZ_00119306 -->

    <owl:NamedIndividual rdf:about="http://purl.obolibrary.org/obo/GAZ_00119306">
        <rdf:type rdf:resource="http://purl.obolibrary.org/obo/ENVO_00000004"/>
        <obo:RO_0001025 rdf:resource="http://purl.obolibrary.org/obo/GAZ_00068776"/>
        <obo:IAO_0000115>A district in Perez Zeledon Canton.</obo:IAO_0000115>
        <oboInOwl:hasOBONamespace>GAZ</oboInOwl:hasOBONamespace>
        <oboInOwl:id>GAZ:00119306</oboInOwl:id>
        <rdfs:label>Paramo District</rdfs:label>
    </owl:NamedIndividual>
    


    <!-- http://purl.obolibrary.org/obo/GAZ_00119307 -->

    <owl:NamedIndividual rdf:about="http://purl.obolibrary.org/obo/GAZ_00119307">
        <rdf:type rdf:resource="http://purl.obolibrary.org/obo/ENVO_00000004"/>
        <obo:RO_0001025 rdf:resource="http://purl.obolibrary.org/obo/GAZ_00068776"/>
        <obo:IAO_0000115>A district in Perez Zeledon Canton.</obo:IAO_0000115>
        <oboInOwl:hasOBONamespace>GAZ</oboInOwl:hasOBONamespace>
        <oboInOwl:id>GAZ:00119307</oboInOwl:id>
        <rdfs:label>San Isidro de El General District</rdfs:label>
    </owl:NamedIndividual>
    


    <!-- http://purl.obolibrary.org/obo/GAZ_00119308 -->

    <owl:NamedIndividual rdf:about="http://purl.obolibrary.org/obo/GAZ_00119308">
        <rdf:type rdf:resource="http://purl.obolibrary.org/obo/ENVO_00000004"/>
        <obo:RO_0001025 rdf:resource="http://purl.obolibrary.org/obo/GAZ_00068776"/>
        <obo:IAO_0000115>A district in Perez Zeledon Canton.</obo:IAO_0000115>
        <oboInOwl:hasOBONamespace>GAZ</oboInOwl:hasOBONamespace>
        <oboInOwl:id>GAZ:00119308</oboInOwl:id>
        <rdfs:label>Baru District</rdfs:label>
    </owl:NamedIndividual>
    


    <!-- http://purl.obolibrary.org/obo/GAZ_00119309 -->

    <owl:NamedIndividual rdf:about="http://purl.obolibrary.org/obo/GAZ_00119309">
        <rdf:type rdf:resource="http://purl.obolibrary.org/obo/ENVO_00000004"/>
        <obo:RO_0001025 rdf:resource="http://purl.obolibrary.org/obo/GAZ_00068776"/>
        <obo:IAO_0000115>A district in Perez Zeledon Canton.</obo:IAO_0000115>
        <oboInOwl:hasOBONamespace>GAZ</oboInOwl:hasOBONamespace>
        <oboInOwl:id>GAZ:00119309</oboInOwl:id>
        <rdfs:label>Cajon District</rdfs:label>
    </owl:NamedIndividual>
    


    <!-- http://purl.obolibrary.org/obo/GAZ_00119310 -->

    <owl:NamedIndividual rdf:about="http://purl.obolibrary.org/obo/GAZ_00119310">
        <rdf:type rdf:resource="http://purl.obolibrary.org/obo/ENVO_00000004"/>
        <obo:RO_0001025 rdf:resource="http://purl.obolibrary.org/obo/GAZ_00068776"/>
        <obo:IAO_0000115>A district in Perez Zeledon Canton.</obo:IAO_0000115>
        <oboInOwl:hasOBONamespace>GAZ</oboInOwl:hasOBONamespace>
        <oboInOwl:id>GAZ:00119310</oboInOwl:id>
        <rdfs:label>San Pedro District</rdfs:label>
    </owl:NamedIndividual>
    


    <!-- http://purl.obolibrary.org/obo/GAZ_00119311 -->

    <owl:NamedIndividual rdf:about="http://purl.obolibrary.org/obo/GAZ_00119311">
        <rdf:type rdf:resource="http://purl.obolibrary.org/obo/ENVO_00000004"/>
        <obo:RO_0001025 rdf:resource="http://purl.obolibrary.org/obo/GAZ_00068776"/>
        <obo:IAO_0000115>A district in Perez Zeledon Canton.</obo:IAO_0000115>
        <oboInOwl:hasOBONamespace>GAZ</oboInOwl:hasOBONamespace>
        <oboInOwl:id>GAZ:00119311</oboInOwl:id>
        <rdfs:label>Rivas District</rdfs:label>
    </owl:NamedIndividual>
    


    <!-- http://purl.obolibrary.org/obo/GAZ_00119312 -->

    <owl:NamedIndividual rdf:about="http://purl.obolibrary.org/obo/GAZ_00119312">
        <rdf:type rdf:resource="http://purl.obolibrary.org/obo/ENVO_00000004"/>
        <obo:RO_0001025 rdf:resource="http://purl.obolibrary.org/obo/GAZ_00068776"/>
        <obo:IAO_0000115>A district in Perez Zeledon Canton.</obo:IAO_0000115>
        <oboInOwl:hasOBONamespace>GAZ</oboInOwl:hasOBONamespace>
        <oboInOwl:id>GAZ:00119312</oboInOwl:id>
        <rdfs:label>Platanares District</rdfs:label>
    </owl:NamedIndividual>
    


    <!-- http://purl.obolibrary.org/obo/GAZ_00119313 -->

    <owl:NamedIndividual rdf:about="http://purl.obolibrary.org/obo/GAZ_00119313">
        <rdf:type rdf:resource="http://purl.obolibrary.org/obo/ENVO_00000004"/>
        <obo:RO_0001025 rdf:resource="http://purl.obolibrary.org/obo/GAZ_00068776"/>
        <obo:IAO_0000115>A district in Perez Zeledon Canton.</obo:IAO_0000115>
        <oboInOwl:hasOBONamespace>GAZ</oboInOwl:hasOBONamespace>
        <oboInOwl:id>GAZ:00119313</oboInOwl:id>
        <rdfs:label>General District</rdfs:label>
    </owl:NamedIndividual>
    


    <!-- http://purl.obolibrary.org/obo/GAZ_00119314 -->

    <owl:NamedIndividual rdf:about="http://purl.obolibrary.org/obo/GAZ_00119314">
        <rdf:type rdf:resource="http://purl.obolibrary.org/obo/ENVO_00000004"/>
        <obo:RO_0001025 rdf:resource="http://purl.obolibrary.org/obo/GAZ_00068776"/>
        <obo:IAO_0000115>A district in Perez Zeledon Canton.</obo:IAO_0000115>
        <oboInOwl:hasOBONamespace>GAZ</oboInOwl:hasOBONamespace>
        <oboInOwl:id>GAZ:00119314</oboInOwl:id>
        <rdfs:label>Rio Nuevo District</rdfs:label>
    </owl:NamedIndividual>
    


    <!-- http://purl.obolibrary.org/obo/GAZ_00119315 -->

    <owl:NamedIndividual rdf:about="http://purl.obolibrary.org/obo/GAZ_00119315">
        <rdf:type rdf:resource="http://purl.obolibrary.org/obo/ENVO_00000004"/>
        <obo:RO_0001025 rdf:resource="http://purl.obolibrary.org/obo/GAZ_00068765"/>
        <obo:IAO_0000115>A district in Leon Cortes Canton.</obo:IAO_0000115>
        <oboInOwl:hasOBONamespace>GAZ</oboInOwl:hasOBONamespace>
        <oboInOwl:id>GAZ:00119315</oboInOwl:id>
        <rdfs:label>Llano Bonito District</rdfs:label>
    </owl:NamedIndividual>
    


    <!-- http://purl.obolibrary.org/obo/GAZ_00119316 -->

    <owl:NamedIndividual rdf:about="http://purl.obolibrary.org/obo/GAZ_00119316">
        <rdf:type rdf:resource="http://purl.obolibrary.org/obo/ENVO_00000004"/>
        <obo:RO_0001025 rdf:resource="http://purl.obolibrary.org/obo/GAZ_00068765"/>
        <obo:IAO_0000115>A district in Leon Cortes Canton.</obo:IAO_0000115>
        <oboInOwl:hasOBONamespace>GAZ</oboInOwl:hasOBONamespace>
        <oboInOwl:id>GAZ:00119316</oboInOwl:id>
        <rdfs:label>San Antonio District</rdfs:label>
    </owl:NamedIndividual>
    


    <!-- http://purl.obolibrary.org/obo/GAZ_00119317 -->

    <owl:NamedIndividual rdf:about="http://purl.obolibrary.org/obo/GAZ_00119317">
        <rdf:type rdf:resource="http://purl.obolibrary.org/obo/ENVO_00000004"/>
        <obo:RO_0001025 rdf:resource="http://purl.obolibrary.org/obo/GAZ_00068765"/>
        <obo:IAO_0000115>A district in Leon Cortes Canton.</obo:IAO_0000115>
        <oboInOwl:hasOBONamespace>GAZ</oboInOwl:hasOBONamespace>
        <oboInOwl:id>GAZ:00119317</oboInOwl:id>
        <rdfs:label>San Pablo District</rdfs:label>
    </owl:NamedIndividual>
    


    <!-- http://purl.obolibrary.org/obo/GAZ_00119318 -->

    <owl:NamedIndividual rdf:about="http://purl.obolibrary.org/obo/GAZ_00119318">
        <rdf:type rdf:resource="http://purl.obolibrary.org/obo/ENVO_00000004"/>
        <obo:RO_0001025 rdf:resource="http://purl.obolibrary.org/obo/GAZ_00068765"/>
        <obo:IAO_0000115>A district in Leon Cortes Canton.</obo:IAO_0000115>
        <oboInOwl:hasOBONamespace>GAZ</oboInOwl:hasOBONamespace>
        <oboInOwl:id>GAZ:00119318</oboInOwl:id>
        <rdfs:label>San Andres District</rdfs:label>
    </owl:NamedIndividual>
    


    <!-- http://purl.obolibrary.org/obo/GAZ_00119319 -->

    <owl:NamedIndividual rdf:about="http://purl.obolibrary.org/obo/GAZ_00119319">
        <rdf:type rdf:resource="http://purl.obolibrary.org/obo/ENVO_00000004"/>
        <obo:RO_0001025 rdf:resource="http://purl.obolibrary.org/obo/GAZ_00068765"/>
        <obo:IAO_0000115>A district in Leon Cortes Canton.</obo:IAO_0000115>
        <oboInOwl:hasOBONamespace>GAZ</oboInOwl:hasOBONamespace>
        <oboInOwl:id>GAZ:00119319</oboInOwl:id>
        <rdfs:label>San Isidro District</rdfs:label>
    </owl:NamedIndividual>
    


    <!-- http://purl.obolibrary.org/obo/GAZ_00119320 -->

    <owl:NamedIndividual rdf:about="http://purl.obolibrary.org/obo/GAZ_00119320">
        <rdf:type rdf:resource="http://purl.obolibrary.org/obo/ENVO_00000004"/>
        <obo:RO_0001025 rdf:resource="http://purl.obolibrary.org/obo/GAZ_00068765"/>
        <obo:IAO_0000115>A district in Leon Cortes Canton.</obo:IAO_0000115>
        <oboInOwl:hasOBONamespace>GAZ</oboInOwl:hasOBONamespace>
        <oboInOwl:id>GAZ:00119320</oboInOwl:id>
        <rdfs:label>Santa Cruz District</rdfs:label>
    </owl:NamedIndividual>
    


    <!-- http://purl.obolibrary.org/obo/GAZ_00144842 -->

    <owl:NamedIndividual rdf:about="http://purl.obolibrary.org/obo/GAZ_00144842">
        <obo:RO_0001025 rdf:resource="http://purl.obolibrary.org/obo/GAZ_00051984"/>
        <obo:IAO_0000115>A very acid crater lake.</obo:IAO_0000115>
        <oboInOwl:hasOBONamespace>GAZ</oboInOwl:hasOBONamespace>
        <oboInOwl:id>GAZ:00144842</oboInOwl:id>
        <rdfs:label>Rincon de la Vieja Crater Lake</rdfs:label>
    </owl:NamedIndividual>
    


    <!-- http://purl.obolibrary.org/obo/GAZ_00145349 -->

    <owl:NamedIndividual rdf:about="http://purl.obolibrary.org/obo/GAZ_00145349">
        <rdf:type rdf:resource="http://purl.obolibrary.org/obo/ENVO_00000032"/>
        <obo:RO_0001025 rdf:resource="http://purl.obolibrary.org/obo/GAZ_00003210"/>
        <obo:IAO_0000115>A large gulf off the northwestern coast of Costa Rica, in the Guanacaste Province.</obo:IAO_0000115>
        <oboInOwl:hasOBONamespace>GAZ</oboInOwl:hasOBONamespace>
        <oboInOwl:id>GAZ:00145349</oboInOwl:id>
        <rdfs:label>Gulf of Papagayo</rdfs:label>
    </owl:NamedIndividual>
    


    <!-- http://purl.obolibrary.org/obo/GAZ_00146617 -->

    <owl:NamedIndividual rdf:about="http://purl.obolibrary.org/obo/GAZ_00146617">
        <obo:RO_0001025 rdf:resource="http://purl.obolibrary.org/obo/GAZ_00068737"/>
        <obo:IAO_0000115>A small bay on the north side of the Osa Peninsula on the coast of southwestern Costa Rica.</obo:IAO_0000115>
        <oboInOwl:hasOBONamespace>GAZ</oboInOwl:hasOBONamespace>
        <oboInOwl:id>GAZ:00146617</oboInOwl:id>
        <rdfs:label>Bahia Drake</rdfs:label>
    </owl:NamedIndividual>
    


    <!-- http://purl.obolibrary.org/obo/GAZ_00247671 -->

    <owl:NamedIndividual rdf:about="http://purl.obolibrary.org/obo/GAZ_00247671">
        <obo:RO_0001025 rdf:resource="http://purl.obolibrary.org/obo/GAZ_00247802"/>
        <obo:IAO_0000115>A seasonal lake.</obo:IAO_0000115>
        <oboInOwl:hasOBONamespace>GAZ</oboInOwl:hasOBONamespace>
        <oboInOwl:id>GAZ:00247671</oboInOwl:id>
        <rdfs:label>Laguna Palo Verde</rdfs:label>
    </owl:NamedIndividual>
    


    <!-- http://purl.obolibrary.org/obo/GAZ_00247799 -->

    <owl:NamedIndividual rdf:about="http://purl.obolibrary.org/obo/GAZ_00247799">
        <obo:RO_0001025 rdf:resource="http://purl.obolibrary.org/obo/GAZ_00068812"/>
        <obo:IAO_0000115>A seasonal lake.</obo:IAO_0000115>
        <oboInOwl:hasOBONamespace>GAZ</oboInOwl:hasOBONamespace>
        <oboInOwl:id>GAZ:00247799</oboInOwl:id>
        <rdfs:label>Laguna Nicaragua</rdfs:label>
    </owl:NamedIndividual>
    


    <!-- http://purl.obolibrary.org/obo/GAZ_00247800 -->

    <owl:NamedIndividual rdf:about="http://purl.obolibrary.org/obo/GAZ_00247800">
        <obo:RO_0001025 rdf:resource="http://purl.obolibrary.org/obo/GAZ_00247799"/>
        <obo:IAO_0000115>An island.</obo:IAO_0000115>
        <oboInOwl:hasOBONamespace>GAZ</oboInOwl:hasOBONamespace>
        <oboInOwl:id>GAZ:00247800</oboInOwl:id>
        <rdfs:label>Isla San Pablo</rdfs:label>
    </owl:NamedIndividual>
    


    <!-- http://purl.obolibrary.org/obo/GAZ_00247801 -->

    <owl:NamedIndividual rdf:about="http://purl.obolibrary.org/obo/GAZ_00247801">
        <obo:RO_0001025 rdf:resource="http://purl.obolibrary.org/obo/GAZ_00247799"/>
        <obo:IAO_0000115>An island.</obo:IAO_0000115>
        <oboInOwl:hasOBONamespace>GAZ</oboInOwl:hasOBONamespace>
        <oboInOwl:id>GAZ:00247801</oboInOwl:id>
        <rdfs:label>Isla Pajaros</rdfs:label>
    </owl:NamedIndividual>
    


    <!-- http://purl.obolibrary.org/obo/GAZ_00247802 -->

    <owl:NamedIndividual rdf:about="http://purl.obolibrary.org/obo/GAZ_00247802">
        <obo:RO_0001025 rdf:resource="http://purl.obolibrary.org/obo/GAZ_00003210"/>
        <obo:RO_0001025 rdf:resource="http://purl.obolibrary.org/obo/GAZ_00068682"/>
        <obo:IAO_0000115>A protected area.</obo:IAO_0000115>
        <oboInOwl:hasOBONamespace>GAZ</oboInOwl:hasOBONamespace>
        <oboInOwl:id>GAZ:00247802</oboInOwl:id>
        <rdfs:label>Dr. Rafael Lucas Rodriguez Caballero National Wildlife Refuge</rdfs:label>
    </owl:NamedIndividual>
    


    <!-- http://purl.obolibrary.org/obo/GAZ_00247803 -->

    <owl:NamedIndividual rdf:about="http://purl.obolibrary.org/obo/GAZ_00247803">
        <obo:RO_0001025 rdf:resource="http://purl.obolibrary.org/obo/GAZ_00068815"/>
        <obo:IAO_0000115>A seasonal freshwater lake.</obo:IAO_0000115>
        <oboInOwl:hasOBONamespace>GAZ</oboInOwl:hasOBONamespace>
        <oboInOwl:id>GAZ:00247803</oboInOwl:id>
        <rdfs:label>Laguna Mata Redonda</rdfs:label>
    </owl:NamedIndividual>
    


    <!-- http://purl.obolibrary.org/obo/GAZ_00247804 -->

    <owl:NamedIndividual rdf:about="http://purl.obolibrary.org/obo/GAZ_00247804">
        <obo:RO_0001025 rdf:resource="http://purl.obolibrary.org/obo/GAZ_00068802"/>
        <obo:IAO_0000115>A fresh/brackish lake on the S bank of the Rio Tempisque.</obo:IAO_0000115>
        <oboInOwl:hasOBONamespace>GAZ</oboInOwl:hasOBONamespace>
        <oboInOwl:id>GAZ:00247804</oboInOwl:id>
        <rdfs:label>Laguna Zonzapote</rdfs:label>
    </owl:NamedIndividual>
    


    <!-- http://purl.obolibrary.org/obo/GAZ_00247805 -->

    <owl:NamedIndividual rdf:about="http://purl.obolibrary.org/obo/GAZ_00247805">
        <obo:RO_0001025 rdf:resource="http://purl.obolibrary.org/obo/GAZ_00003210"/>
        <obo:IAO_0000115>Saltpans.</obo:IAO_0000115>
        <oboInOwl:hasOBONamespace>GAZ</oboInOwl:hasOBONamespace>
        <oboInOwl:id>GAZ:00247805</oboInOwl:id>
        <rdfs:label>Salina Bonilla</rdfs:label>
    </owl:NamedIndividual>
    


    <!-- http://purl.obolibrary.org/obo/GAZ_00247806 -->

    <owl:NamedIndividual rdf:about="http://purl.obolibrary.org/obo/GAZ_00247806">
        <obo:RO_0001025 rdf:resource="http://purl.obolibrary.org/obo/GAZ_00003210"/>
        <obo:IAO_0000115>Brackish coastal marshes.</obo:IAO_0000115>
        <oboInOwl:hasOBONamespace>GAZ</oboInOwl:hasOBONamespace>
        <oboInOwl:id>GAZ:00247806</oboInOwl:id>
        <rdfs:label>Estero Piedras</rdfs:label>
    </owl:NamedIndividual>
    


    <!-- http://purl.obolibrary.org/obo/GAZ_00247807 -->

    <owl:NamedIndividual rdf:about="http://purl.obolibrary.org/obo/GAZ_00247807">
        <obo:RO_0001025 rdf:resource="http://purl.obolibrary.org/obo/GAZ_00003209"/>
        <obo:IAO_0000115>Brackish coastal lagoons. Located near Barranca.</obo:IAO_0000115>
        <oboInOwl:hasOBONamespace>GAZ</oboInOwl:hasOBONamespace>
        <oboInOwl:id>GAZ:00247807</oboInOwl:id>
        <rdfs:label>Estero Mata de Limon</rdfs:label>
    </owl:NamedIndividual>
    


    <!-- http://purl.obolibrary.org/obo/GAZ_00247808 -->

    <owl:NamedIndividual rdf:about="http://purl.obolibrary.org/obo/GAZ_00247808">
        <obo:RO_0001025 rdf:resource="http://purl.obolibrary.org/obo/GAZ_00068739"/>
        <obo:IAO_0000115>A freshwater lake.</obo:IAO_0000115>
        <oboInOwl:hasOBONamespace>GAZ</oboInOwl:hasOBONamespace>
        <oboInOwl:id>GAZ:00247808</oboInOwl:id>
        <rdfs:label>Laguna Corcovado</rdfs:label>
    </owl:NamedIndividual>
    


    <!-- http://purl.obolibrary.org/obo/GAZ_00247809 -->

    <owl:NamedIndividual rdf:about="http://purl.obolibrary.org/obo/GAZ_00247809">
        <obo:RO_0001025 rdf:resource="http://purl.obolibrary.org/obo/GAZ_00003206"/>
        <obo:RO_0001025 rdf:resource="http://purl.obolibrary.org/obo/GAZ_00068876"/>
        <obo:IAO_0000115>A freshwater lake.</obo:IAO_0000115>
        <oboInOwl:hasOBONamespace>GAZ</oboInOwl:hasOBONamespace>
        <oboInOwl:id>GAZ:00247809</oboInOwl:id>
        <rdfs:label>Lago Dabagri</rdfs:label>
    </owl:NamedIndividual>
    


    <!-- http://purl.obolibrary.org/obo/GAZ_00247810 -->

    <owl:NamedIndividual rdf:about="http://purl.obolibrary.org/obo/GAZ_00247810">
        <obo:RO_0001025 rdf:resource="http://purl.obolibrary.org/obo/GAZ_00003206"/>
        <obo:IAO_0000115>A brackish lake. Located on the Caribbean coast near the Panamanian border.</obo:IAO_0000115>
        <oboInOwl:hasOBONamespace>GAZ</oboInOwl:hasOBONamespace>
        <oboInOwl:id>GAZ:00247810</oboInOwl:id>
        <rdfs:label>Laguna Gandoca</rdfs:label>
    </owl:NamedIndividual>
    


    <!-- http://purl.obolibrary.org/obo/GAZ_00247811 -->

    <owl:NamedIndividual rdf:about="http://purl.obolibrary.org/obo/GAZ_00247811">
        <obo:RO_0001025 rdf:resource="http://purl.obolibrary.org/obo/GAZ_00068725"/>
        <obo:IAO_0000115>A complex of interconnexted freshwater lakes and marshes, brackish coastal lagoons and marshes and palm swamps behinf a sandy beach. The lagoons are subject to tidal influence.</obo:IAO_0000115>
        <oboInOwl:hasOBONamespace>GAZ</oboInOwl:hasOBONamespace>
        <oboInOwl:id>GAZ:00247811</oboInOwl:id>
        <rdfs:label>Barra del Colorado</rdfs:label>
    </owl:NamedIndividual>
    


    <!-- http://purl.obolibrary.org/obo/GAZ_00264514 -->

    <owl:NamedIndividual rdf:about="http://purl.obolibrary.org/obo/GAZ_00264514">
        <obo:RO_0001025 rdf:resource="http://purl.obolibrary.org/obo/GAZ_00003210"/>
        <obo:IAO_0000115>A research station located in the Guanacaste Province of Costa Rica.</obo:IAO_0000115>
        <oboInOwl:hasOBONamespace>GAZ</oboInOwl:hasOBONamespace>
        <oboInOwl:id>GAZ:00264514</oboInOwl:id>
        <rdfs:label>Palo Verde Biological Station</rdfs:label>
    </owl:NamedIndividual>
    


    <!-- http://purl.obolibrary.org/obo/GAZ_00264518 -->

    <owl:NamedIndividual rdf:about="http://purl.obolibrary.org/obo/GAZ_00264518">
        <obo:RO_0001025 rdf:resource="http://purl.obolibrary.org/obo/GAZ_00003208"/>
        <obo:IAO_0000115>A river. A tributary of the San Juan River.</obo:IAO_0000115>
        <oboInOwl:hasOBONamespace>GAZ</oboInOwl:hasOBONamespace>
        <oboInOwl:id>GAZ:00264518</oboInOwl:id>
        <rdfs:label>Rio Sarapiqui</rdfs:label>
    </owl:NamedIndividual>
    


    <!-- http://purl.obolibrary.org/obo/GAZ_00264519 -->

    <owl:NamedIndividual rdf:about="http://purl.obolibrary.org/obo/GAZ_00264519">
        <obo:RO_0001025 rdf:resource="http://purl.obolibrary.org/obo/GAZ_00003208"/>
        <obo:IAO_0000115>A river.</obo:IAO_0000115>
        <oboInOwl:hasOBONamespace>GAZ</oboInOwl:hasOBONamespace>
        <oboInOwl:id>GAZ:00264519</oboInOwl:id>
        <rdfs:label>Rio Toro</rdfs:label>
    </owl:NamedIndividual>
    


    <!-- http://purl.obolibrary.org/obo/GAZ_00264520 -->

    <owl:NamedIndividual rdf:about="http://purl.obolibrary.org/obo/GAZ_00264520">
        <obo:RO_0001025 rdf:resource="http://purl.obolibrary.org/obo/GAZ_00003208"/>
        <obo:IAO_0000115>A river.</obo:IAO_0000115>
        <oboInOwl:hasOBONamespace>GAZ</oboInOwl:hasOBONamespace>
        <oboInOwl:id>GAZ:00264520</oboInOwl:id>
        <rdfs:label>Rio Sucio</rdfs:label>
    </owl:NamedIndividual>
    


    <!-- http://purl.obolibrary.org/obo/GAZ_00264521 -->

    <owl:NamedIndividual rdf:about="http://purl.obolibrary.org/obo/GAZ_00264521">
        <obo:RO_0001025 rdf:resource="http://purl.obolibrary.org/obo/GAZ_00003205"/>
        <oboInOwl:hasOBONamespace>GAZ</oboInOwl:hasOBONamespace>
        <oboInOwl:id>GAZ:00264521</oboInOwl:id>
        <rdfs:label>Rio San Carlos</rdfs:label>
    </owl:NamedIndividual>
    


    <!-- http://purl.obolibrary.org/obo/GAZ_00264525 -->

    <owl:NamedIndividual rdf:about="http://purl.obolibrary.org/obo/GAZ_00264525">
        <obo:RO_0001025 rdf:resource="http://purl.obolibrary.org/obo/GAZ_00003205"/>
        <obo:IAO_0000115>A river.</obo:IAO_0000115>
        <oboInOwl:hasOBONamespace>GAZ</oboInOwl:hasOBONamespace>
        <oboInOwl:id>GAZ:00264525</oboInOwl:id>
        <rdfs:label>Rio Celeste</rdfs:label>
    </owl:NamedIndividual>
    


    <!-- http://purl.obolibrary.org/obo/GAZ_00264526 -->

    <owl:NamedIndividual rdf:about="http://purl.obolibrary.org/obo/GAZ_00264526">
        <obo:RO_0001025 rdf:resource="http://purl.obolibrary.org/obo/GAZ_00003205"/>
        <obo:IAO_0000115>A river.</obo:IAO_0000115>
        <oboInOwl:hasOBONamespace>GAZ</oboInOwl:hasOBONamespace>
        <oboInOwl:id>GAZ:00264526</oboInOwl:id>
        <rdfs:label>Rio Sabogal</rdfs:label>
    </owl:NamedIndividual>
    


    <!-- http://purl.obolibrary.org/obo/GAZ_00264527 -->

    <owl:NamedIndividual rdf:about="http://purl.obolibrary.org/obo/GAZ_00264527">
        <obo:RO_0001025 rdf:resource="http://purl.obolibrary.org/obo/GAZ_00068891"/>
        <obo:IAO_0000115>A National Park in the northern part of Costa Rica, which forms part of the Arenal Tilaran Conservation Area.</obo:IAO_0000115>
        <oboInOwl:hasOBONamespace>GAZ</oboInOwl:hasOBONamespace>
        <oboInOwl:id>GAZ:00264527</oboInOwl:id>
        <rdfs:label>Parque Nacional Volcan Tenorio</rdfs:label>
    </owl:NamedIndividual>
    


    <!-- http://purl.obolibrary.org/obo/GAZ_00264531 -->

    <owl:NamedIndividual rdf:about="http://purl.obolibrary.org/obo/GAZ_00264531">
        <obo:RO_0001025 rdf:resource="http://purl.obolibrary.org/obo/GAZ_00003206"/>
        <obo:IAO_0000115>A river. Drains to the Atlantic Ocean.</obo:IAO_0000115>
        <oboInOwl:hasOBONamespace>GAZ</oboInOwl:hasOBONamespace>
        <oboInOwl:id>GAZ:00264531</oboInOwl:id>
        <rdfs:label>Rio Suerte</rdfs:label>
    </owl:NamedIndividual>
    


    <!-- http://purl.obolibrary.org/obo/GAZ_00264532 -->

    <owl:NamedIndividual rdf:about="http://purl.obolibrary.org/obo/GAZ_00264532">
        <obo:RO_0001025 rdf:resource="http://purl.obolibrary.org/obo/GAZ_00003206"/>
        <oboInOwl:hasOBONamespace>GAZ</oboInOwl:hasOBONamespace>
        <oboInOwl:id>GAZ:00264532</oboInOwl:id>
        <rdfs:label>Rio Tortuguero</rdfs:label>
    </owl:NamedIndividual>
    


    <!-- http://purl.obolibrary.org/obo/GAZ_00264534 -->

    <owl:NamedIndividual rdf:about="http://purl.obolibrary.org/obo/GAZ_00264534">
        <obo:RO_0001025 rdf:resource="http://purl.obolibrary.org/obo/GAZ_00003206"/>
        <obo:IAO_0000115>A river.</obo:IAO_0000115>
        <oboInOwl:hasOBONamespace>GAZ</oboInOwl:hasOBONamespace>
        <oboInOwl:id>GAZ:00264534</oboInOwl:id>
        <rdfs:label>Rio Parismina</rdfs:label>
    </owl:NamedIndividual>
    


    <!-- http://purl.obolibrary.org/obo/GAZ_00264535 -->

    <owl:NamedIndividual rdf:about="http://purl.obolibrary.org/obo/GAZ_00264535">
        <obo:RO_0001025 rdf:resource="http://purl.obolibrary.org/obo/GAZ_00003206"/>
        <obo:IAO_0000115>A river.</obo:IAO_0000115>
        <oboInOwl:hasOBONamespace>GAZ</oboInOwl:hasOBONamespace>
        <oboInOwl:id>GAZ:00264535</oboInOwl:id>
        <rdfs:label>Rio Jimenez</rdfs:label>
    </owl:NamedIndividual>
    


    <!-- http://purl.obolibrary.org/obo/GAZ_00264536 -->

    <owl:NamedIndividual rdf:about="http://purl.obolibrary.org/obo/GAZ_00264536">
        <obo:RO_0001025 rdf:resource="http://purl.obolibrary.org/obo/GAZ_00003211"/>
        <obo:IAO_0000115>A river.</obo:IAO_0000115>
        <oboInOwl:hasOBONamespace>GAZ</oboInOwl:hasOBONamespace>
        <oboInOwl:id>GAZ:00264536</oboInOwl:id>
        <rdfs:label>Rio Atirro</rdfs:label>
    </owl:NamedIndividual>
    


    <!-- http://purl.obolibrary.org/obo/GAZ_00264539 -->

    <owl:NamedIndividual rdf:about="http://purl.obolibrary.org/obo/GAZ_00264539">
        <obo:RO_0001025 rdf:resource="http://purl.obolibrary.org/obo/GAZ_00003206"/>
        <obo:IAO_0000115>A river. Discharges to the Atlantic Ocean.</obo:IAO_0000115>
        <oboInOwl:hasOBONamespace>GAZ</oboInOwl:hasOBONamespace>
        <oboInOwl:id>GAZ:00264539</oboInOwl:id>
        <rdfs:label>Rio Pacuare</rdfs:label>
    </owl:NamedIndividual>
    


    <!-- http://purl.obolibrary.org/obo/GAZ_00264540 -->

    <owl:NamedIndividual rdf:about="http://purl.obolibrary.org/obo/GAZ_00264540">
        <obo:RO_0001025 rdf:resource="http://purl.obolibrary.org/obo/GAZ_00003206"/>
        <obo:IAO_0000115>A river. Discharges to the Atlantic Ocean.</obo:IAO_0000115>
        <oboInOwl:hasOBONamespace>GAZ</oboInOwl:hasOBONamespace>
        <oboInOwl:id>GAZ:00264540</oboInOwl:id>
        <rdfs:label>Rio Matina</rdfs:label>
    </owl:NamedIndividual>
    


    <!-- http://purl.obolibrary.org/obo/GAZ_00264541 -->

    <owl:NamedIndividual rdf:about="http://purl.obolibrary.org/obo/GAZ_00264541">
        <obo:RO_0001025 rdf:resource="http://purl.obolibrary.org/obo/GAZ_00003211"/>
        <obo:IAO_0000115>A reservoir.</obo:IAO_0000115>
        <oboInOwl:hasOBONamespace>GAZ</oboInOwl:hasOBONamespace>
        <oboInOwl:id>GAZ:00264541</oboInOwl:id>
        <rdfs:label>Repressa Hidroelectrica Angostura</rdfs:label>
    </owl:NamedIndividual>
    


    <!-- http://purl.obolibrary.org/obo/GAZ_00264542 -->

    <owl:NamedIndividual rdf:about="http://purl.obolibrary.org/obo/GAZ_00264542">
        <obo:RO_0001025 rdf:resource="http://purl.obolibrary.org/obo/GAZ_00003206"/>
        <obo:IAO_0000115>A river. Discharges to the Atlantic Ocean.</obo:IAO_0000115>
        <oboInOwl:hasOBONamespace>GAZ</oboInOwl:hasOBONamespace>
        <oboInOwl:id>GAZ:00264542</oboInOwl:id>
        <rdfs:label>Rio Banano</rdfs:label>
    </owl:NamedIndividual>
    


    <!-- http://purl.obolibrary.org/obo/GAZ_00264543 -->

    <owl:NamedIndividual rdf:about="http://purl.obolibrary.org/obo/GAZ_00264543">
        <obo:RO_0001025 rdf:resource="http://purl.obolibrary.org/obo/GAZ_00003206"/>
        <obo:IAO_0000115>A river. Discharges to the Atlantic Ocean.</obo:IAO_0000115>
        <oboInOwl:hasOBONamespace>GAZ</oboInOwl:hasOBONamespace>
        <oboInOwl:id>GAZ:00264543</oboInOwl:id>
        <rdfs:label>Rio Estrella</rdfs:label>
    </owl:NamedIndividual>
    


    <!-- http://purl.obolibrary.org/obo/GAZ_00264544 -->

    <owl:NamedIndividual rdf:about="http://purl.obolibrary.org/obo/GAZ_00264544">
        <obo:RO_0001025 rdf:resource="http://purl.obolibrary.org/obo/GAZ_00003211"/>
        <obo:IAO_0000115>A reservoir. Impounded by Embalse Cachi.</obo:IAO_0000115>
        <oboInOwl:hasOBONamespace>GAZ</oboInOwl:hasOBONamespace>
        <oboInOwl:id>GAZ:00264544</oboInOwl:id>
        <rdfs:label>Lago de Cachi</rdfs:label>
    </owl:NamedIndividual>
    


    <!-- http://purl.obolibrary.org/obo/GAZ_00264545 -->

    <owl:NamedIndividual rdf:about="http://purl.obolibrary.org/obo/GAZ_00264545">
        <obo:RO_0001025 rdf:resource="http://purl.obolibrary.org/obo/GAZ_00003211"/>
        <obo:IAO_0000115>A dam. Impounds Lago de Cachi.</obo:IAO_0000115>
        <oboInOwl:hasOBONamespace>GAZ</oboInOwl:hasOBONamespace>
        <oboInOwl:id>GAZ:00264545</oboInOwl:id>
        <rdfs:label>Represa Cachi</rdfs:label>
    </owl:NamedIndividual>
    


    <!-- http://purl.obolibrary.org/obo/GAZ_00264550 -->

    <owl:NamedIndividual rdf:about="http://purl.obolibrary.org/obo/GAZ_00264550">
        <obo:RO_0001025 rdf:resource="http://purl.obolibrary.org/obo/GAZ_00003210"/>
        <obo:IAO_0000115>A river in the Guanacaste Province of Costa Rica. The estuary is adjacent to the town of Tamarindo.</obo:IAO_0000115>
        <oboInOwl:hasOBONamespace>GAZ</oboInOwl:hasOBONamespace>
        <oboInOwl:id>GAZ:00264550</oboInOwl:id>
        <rdfs:label>Rio Tamarindo</rdfs:label>
    </owl:NamedIndividual>
    


    <!-- http://purl.obolibrary.org/obo/GAZ_00264551 -->

    <owl:NamedIndividual rdf:about="http://purl.obolibrary.org/obo/GAZ_00264551">
        <obo:RO_0001025 rdf:resource="http://purl.obolibrary.org/obo/GAZ_00003210"/>
        <obo:IAO_0000115>A river. Drains to the Pacific Ocean.</obo:IAO_0000115>
        <oboInOwl:hasOBONamespace>GAZ</oboInOwl:hasOBONamespace>
        <oboInOwl:id>GAZ:00264551</oboInOwl:id>
        <rdfs:label>Rio Nosara</rdfs:label>
    </owl:NamedIndividual>
    


    <!-- http://purl.obolibrary.org/obo/GAZ_00264552 -->

    <owl:NamedIndividual rdf:about="http://purl.obolibrary.org/obo/GAZ_00264552">
        <obo:RO_0001025 rdf:resource="http://purl.obolibrary.org/obo/GAZ_00068697"/>
        <oboInOwl:hasOBONamespace>GAZ</oboInOwl:hasOBONamespace>
        <oboInOwl:id>GAZ:00264552</oboInOwl:id>
        <rdfs:label>Isla Alcatraz</rdfs:label>
    </owl:NamedIndividual>
    


    <!-- http://purl.obolibrary.org/obo/GAZ_00264553 -->

    <owl:NamedIndividual rdf:about="http://purl.obolibrary.org/obo/GAZ_00264553">
        <obo:RO_0001025 rdf:resource="http://purl.obolibrary.org/obo/GAZ_00068697"/>
        <oboInOwl:hasOBONamespace>GAZ</oboInOwl:hasOBONamespace>
        <oboInOwl:id>GAZ:00264553</oboInOwl:id>
        <rdfs:label>Isla Tolinga</rdfs:label>
    </owl:NamedIndividual>
    


    <!-- http://purl.obolibrary.org/obo/GAZ_00264554 -->

    <owl:NamedIndividual rdf:about="http://purl.obolibrary.org/obo/GAZ_00264554">
        <obo:RO_0001025 rdf:resource="http://purl.obolibrary.org/obo/GAZ_00068690"/>
        <oboInOwl:hasOBONamespace>GAZ</oboInOwl:hasOBONamespace>
        <oboInOwl:id>GAZ:00264554</oboInOwl:id>
        <rdfs:label>Isla Pan de Azucar</rdfs:label>
    </owl:NamedIndividual>
    


    <!-- http://purl.obolibrary.org/obo/GAZ_00264555 -->

    <owl:NamedIndividual rdf:about="http://purl.obolibrary.org/obo/GAZ_00264555">
        <obo:RO_0001025 rdf:resource="http://purl.obolibrary.org/obo/GAZ_00068690"/>
        <oboInOwl:hasOBONamespace>GAZ</oboInOwl:hasOBONamespace>
        <oboInOwl:id>GAZ:00264555</oboInOwl:id>
        <rdfs:label>Isla Muertos</rdfs:label>
    </owl:NamedIndividual>
    


    <!-- http://purl.obolibrary.org/obo/GAZ_00264556 -->

    <owl:NamedIndividual rdf:about="http://purl.obolibrary.org/obo/GAZ_00264556">
        <obo:RO_0001025 rdf:resource="http://purl.obolibrary.org/obo/GAZ_00068690"/>
        <oboInOwl:hasOBONamespace>GAZ</oboInOwl:hasOBONamespace>
        <oboInOwl:id>GAZ:00264556</oboInOwl:id>
        <rdfs:label>Isla Jesusita</rdfs:label>
    </owl:NamedIndividual>
    


    <!-- http://purl.obolibrary.org/obo/GAZ_00264557 -->

    <owl:NamedIndividual rdf:about="http://purl.obolibrary.org/obo/GAZ_00264557">
        <obo:RO_0001025 rdf:resource="http://purl.obolibrary.org/obo/GAZ_00003210"/>
        <obo:IAO_0000115>A river located entirely in Costa Rica flowing from the Guanacaste Cordillera near the Orosi Volcano and emptying into the Gulf of Nicoya. It passes through the Palo Verde National Park.</obo:IAO_0000115>
        <oboInOwl:hasOBONamespace>GAZ</oboInOwl:hasOBONamespace>
        <oboInOwl:id>GAZ:00264557</oboInOwl:id>
        <rdfs:label>Rio Tempisque</rdfs:label>
    </owl:NamedIndividual>
    


    <!-- http://purl.obolibrary.org/obo/GAZ_00264558 -->

    <owl:NamedIndividual rdf:about="http://purl.obolibrary.org/obo/GAZ_00264558">
        <obo:RO_0001025 rdf:resource="http://purl.obolibrary.org/obo/GAZ_00003210"/>
        <obo:IAO_0000115>A river.</obo:IAO_0000115>
        <oboInOwl:hasOBONamespace>GAZ</oboInOwl:hasOBONamespace>
        <oboInOwl:id>GAZ:00264558</oboInOwl:id>
        <rdfs:label>Rio Bebedero</rdfs:label>
    </owl:NamedIndividual>
    


    <!-- http://purl.obolibrary.org/obo/GAZ_00264559 -->

    <owl:NamedIndividual rdf:about="http://purl.obolibrary.org/obo/GAZ_00264559">
        <obo:RO_0001025 rdf:resource="http://purl.obolibrary.org/obo/GAZ_00003210"/>
        <obo:IAO_0000115>A river.</obo:IAO_0000115>
        <oboInOwl:hasOBONamespace>GAZ</oboInOwl:hasOBONamespace>
        <oboInOwl:id>GAZ:00264559</oboInOwl:id>
        <rdfs:label>Rio Canas [Bebedero]</rdfs:label>
    </owl:NamedIndividual>
    


    <!-- http://purl.obolibrary.org/obo/GAZ_00264560 -->

    <owl:NamedIndividual rdf:about="http://purl.obolibrary.org/obo/GAZ_00264560">
        <obo:RO_0001025 rdf:resource="http://purl.obolibrary.org/obo/GAZ_00003210"/>
        <obo:IAO_0000115>A river.</obo:IAO_0000115>
        <oboInOwl:hasOBONamespace>GAZ</oboInOwl:hasOBONamespace>
        <oboInOwl:id>GAZ:00264560</oboInOwl:id>
        <rdfs:label>Rio Piedras</rdfs:label>
    </owl:NamedIndividual>
    


    <!-- http://purl.obolibrary.org/obo/GAZ_00264562 -->

    <owl:NamedIndividual rdf:about="http://purl.obolibrary.org/obo/GAZ_00264562">
        <obo:RO_0001025 rdf:resource="http://purl.obolibrary.org/obo/GAZ_00003210"/>
        <obo:RO_0001025 rdf:resource="http://purl.obolibrary.org/obo/GAZ_00003211"/>
        <obo:IAO_0000115>A river.</obo:IAO_0000115>
        <oboInOwl:hasOBONamespace>GAZ</oboInOwl:hasOBONamespace>
        <oboInOwl:id>GAZ:00264562</oboInOwl:id>
        <rdfs:label>Rio Tenorio</rdfs:label>
    </owl:NamedIndividual>
    


    <!-- http://purl.obolibrary.org/obo/GAZ_00264563 -->

    <owl:NamedIndividual rdf:about="http://purl.obolibrary.org/obo/GAZ_00264563">
        <obo:RO_0001025 rdf:resource="http://purl.obolibrary.org/obo/GAZ_00003210"/>
        <obo:IAO_0000115>A river.</obo:IAO_0000115>
        <oboInOwl:hasOBONamespace>GAZ</oboInOwl:hasOBONamespace>
        <oboInOwl:id>GAZ:00264563</oboInOwl:id>
        <rdfs:label>Rio Canas [Tempisque]</rdfs:label>
    </owl:NamedIndividual>
    


    <!-- http://purl.obolibrary.org/obo/GAZ_00264564 -->

    <owl:NamedIndividual rdf:about="http://purl.obolibrary.org/obo/GAZ_00264564">
        <obo:RO_0001025 rdf:resource="http://purl.obolibrary.org/obo/GAZ_00003210"/>
        <obo:IAO_0000115>A river.</obo:IAO_0000115>
        <oboInOwl:hasOBONamespace>GAZ</oboInOwl:hasOBONamespace>
        <oboInOwl:id>GAZ:00264564</oboInOwl:id>
        <rdfs:label>Rio Salto</rdfs:label>
    </owl:NamedIndividual>
    


    <!-- http://purl.obolibrary.org/obo/GAZ_00264565 -->

    <owl:NamedIndividual rdf:about="http://purl.obolibrary.org/obo/GAZ_00264565">
        <obo:RO_0001025 rdf:resource="http://purl.obolibrary.org/obo/GAZ_00003210"/>
        <obo:IAO_0000115>A river.</obo:IAO_0000115>
        <oboInOwl:hasOBONamespace>GAZ</oboInOwl:hasOBONamespace>
        <oboInOwl:id>GAZ:00264565</oboInOwl:id>
        <rdfs:label>Rio Liberi</rdfs:label>
    </owl:NamedIndividual>
    


    <!-- http://purl.obolibrary.org/obo/GAZ_00264566 -->

    <owl:NamedIndividual rdf:about="http://purl.obolibrary.org/obo/GAZ_00264566">
        <obo:RO_0001025 rdf:resource="http://purl.obolibrary.org/obo/GAZ_00003210"/>
        <obo:IAO_0000115>A river.</obo:IAO_0000115>
        <oboInOwl:hasOBONamespace>GAZ</oboInOwl:hasOBONamespace>
        <oboInOwl:id>GAZ:00264566</oboInOwl:id>
        <rdfs:label>Rio Colorado</rdfs:label>
    </owl:NamedIndividual>
    


    <!-- http://purl.obolibrary.org/obo/GAZ_00264567 -->

    <owl:NamedIndividual rdf:about="http://purl.obolibrary.org/obo/GAZ_00264567">
        <obo:RO_0001025 rdf:resource="http://purl.obolibrary.org/obo/GAZ_00003209"/>
        <obo:IAO_0000115>A river.</obo:IAO_0000115>
        <oboInOwl:hasOBONamespace>GAZ</oboInOwl:hasOBONamespace>
        <oboInOwl:id>GAZ:00264567</oboInOwl:id>
        <rdfs:label>Rio Abangares</rdfs:label>
    </owl:NamedIndividual>
    


    <!-- http://purl.obolibrary.org/obo/GAZ_00264568 -->

    <owl:NamedIndividual rdf:about="http://purl.obolibrary.org/obo/GAZ_00264568">
        <obo:RO_0001025 rdf:resource="http://purl.obolibrary.org/obo/GAZ_00003209"/>
        <obo:IAO_0000115>A river.</obo:IAO_0000115>
        <oboInOwl:hasOBONamespace>GAZ</oboInOwl:hasOBONamespace>
        <oboInOwl:id>GAZ:00264568</oboInOwl:id>
        <rdfs:label>Rio Lagarto</rdfs:label>
    </owl:NamedIndividual>
    


    <!-- http://purl.obolibrary.org/obo/GAZ_00264569 -->

    <owl:NamedIndividual rdf:about="http://purl.obolibrary.org/obo/GAZ_00264569">
        <obo:RO_0001025 rdf:resource="http://purl.obolibrary.org/obo/GAZ_00003209"/>
        <obo:IAO_0000115>A river.</obo:IAO_0000115>
        <oboInOwl:hasOBONamespace>GAZ</oboInOwl:hasOBONamespace>
        <oboInOwl:id>GAZ:00264569</oboInOwl:id>
        <rdfs:label>Rio Guacimal</rdfs:label>
    </owl:NamedIndividual>
    


    <!-- http://purl.obolibrary.org/obo/GAZ_00264570 -->

    <owl:NamedIndividual rdf:about="http://purl.obolibrary.org/obo/GAZ_00264570">
        <obo:RO_0001025 rdf:resource="http://purl.obolibrary.org/obo/GAZ_00003209"/>
        <obo:IAO_0000115>A river.</obo:IAO_0000115>
        <oboInOwl:hasOBONamespace>GAZ</oboInOwl:hasOBONamespace>
        <oboInOwl:id>GAZ:00264570</oboInOwl:id>
        <rdfs:label>Rio Aranjuez</rdfs:label>
    </owl:NamedIndividual>
    


    <!-- http://purl.obolibrary.org/obo/GAZ_00264572 -->

    <owl:NamedIndividual rdf:about="http://purl.obolibrary.org/obo/GAZ_00264572">
        <obo:RO_0001025 rdf:resource="http://purl.obolibrary.org/obo/GAZ_00003209"/>
        <obo:IAO_0000115>A river.</obo:IAO_0000115>
        <oboInOwl:hasOBONamespace>GAZ</oboInOwl:hasOBONamespace>
        <oboInOwl:id>GAZ:00264572</oboInOwl:id>
        <rdfs:label>Rio Jesus Maria</rdfs:label>
    </owl:NamedIndividual>
    


    <!-- http://purl.obolibrary.org/obo/GAZ_00264577 -->

    <owl:NamedIndividual rdf:about="http://purl.obolibrary.org/obo/GAZ_00264577">
        <obo:RO_0001025 rdf:resource="http://purl.obolibrary.org/obo/GAZ_00003209"/>
        <obo:IAO_0000115>A river.</obo:IAO_0000115>
        <oboInOwl:hasOBONamespace>GAZ</oboInOwl:hasOBONamespace>
        <oboInOwl:id>GAZ:00264577</oboInOwl:id>
        <rdfs:label>Rio Terraba</rdfs:label>
    </owl:NamedIndividual>
    


    <!-- http://purl.obolibrary.org/obo/GAZ_00264578 -->

    <owl:NamedIndividual rdf:about="http://purl.obolibrary.org/obo/GAZ_00264578">
        <obo:RO_0001025 rdf:resource="http://purl.obolibrary.org/obo/GAZ_00003209"/>
        <obo:IAO_0000115>A river.</obo:IAO_0000115>
        <oboInOwl:hasOBONamespace>GAZ</oboInOwl:hasOBONamespace>
        <oboInOwl:id>GAZ:00264578</oboInOwl:id>
        <rdfs:label>Rio Coto Brus</rdfs:label>
    </owl:NamedIndividual>
    


    <!-- http://purl.obolibrary.org/obo/GAZ_00264581 -->

    <owl:NamedIndividual rdf:about="http://purl.obolibrary.org/obo/GAZ_00264581">
        <obo:RO_0001025 rdf:resource="http://purl.obolibrary.org/obo/GAZ_00003209"/>
        <obo:IAO_0000115>A river.</obo:IAO_0000115>
        <oboInOwl:hasOBONamespace>GAZ</oboInOwl:hasOBONamespace>
        <oboInOwl:id>GAZ:00264581</oboInOwl:id>
        <rdfs:label>Rio Sierpe</rdfs:label>
    </owl:NamedIndividual>
    


    <!-- http://purl.obolibrary.org/obo/GAZ_00264582 -->

    <owl:NamedIndividual rdf:about="http://purl.obolibrary.org/obo/GAZ_00264582">
        <obo:RO_0001025 rdf:resource="http://purl.obolibrary.org/obo/GAZ_00003209"/>
        <obo:IAO_0000115>A river.</obo:IAO_0000115>
        <oboInOwl:hasOBONamespace>GAZ</oboInOwl:hasOBONamespace>
        <oboInOwl:id>GAZ:00264582</oboInOwl:id>
        <rdfs:label>Rio Coto Colorado</rdfs:label>
    </owl:NamedIndividual>
    


    <!-- http://purl.obolibrary.org/obo/GAZ_00264583 -->

    <owl:NamedIndividual rdf:about="http://purl.obolibrary.org/obo/GAZ_00264583">
        <obo:RO_0001025 rdf:resource="http://purl.obolibrary.org/obo/GAZ_00003210"/>
        <obo:IAO_0000115>A peninsula.</obo:IAO_0000115>
        <oboInOwl:hasOBONamespace>GAZ</oboInOwl:hasOBONamespace>
        <oboInOwl:id>GAZ:00264583</oboInOwl:id>
        <rdfs:label>Papagayo Peninsula</rdfs:label>
    </owl:NamedIndividual>
    


    <!-- http://purl.obolibrary.org/obo/GAZ_00267207 -->

    <owl:NamedIndividual rdf:about="http://purl.obolibrary.org/obo/GAZ_00267207">
        <obo:IAO_0000115>A river.</obo:IAO_0000115>
        <oboInOwl:hasOBONamespace>GAZ</oboInOwl:hasOBONamespace>
        <oboInOwl:id>GAZ:00267207</oboInOwl:id>
        <rdfs:label>Rio Sabo Jose</rdfs:label>
    </owl:NamedIndividual>
    


    <!-- http://purl.obolibrary.org/obo/GAZ_00267208 -->

    <owl:NamedIndividual rdf:about="http://purl.obolibrary.org/obo/GAZ_00267208">
        <obo:IAO_0000115>A river.</obo:IAO_0000115>
        <oboInOwl:hasOBONamespace>GAZ</oboInOwl:hasOBONamespace>
        <oboInOwl:id>GAZ:00267208</oboInOwl:id>
        <rdfs:label>Rio Santa Cruz</rdfs:label>
    </owl:NamedIndividual>
    


    <!-- http://purl.obolibrary.org/obo/GAZ_00267750 -->

    <owl:NamedIndividual rdf:about="http://purl.obolibrary.org/obo/GAZ_00267750">
        <obo:IAO_0000115>The extremity of the Peninsula de Burica.</obo:IAO_0000115>
        <oboInOwl:hasOBONamespace>GAZ</oboInOwl:hasOBONamespace>
        <oboInOwl:id>GAZ:00267750</oboInOwl:id>
        <rdfs:label>Punta Burica</rdfs:label>
    </owl:NamedIndividual>
    


    <!-- http://purl.obolibrary.org/obo/GAZ_00267751 -->

    <owl:NamedIndividual rdf:about="http://purl.obolibrary.org/obo/GAZ_00267751">
        <obo:IAO_0000115>A protected area in Costa Rica and Panama.</obo:IAO_0000115>
        <oboInOwl:hasOBONamespace>GAZ</oboInOwl:hasOBONamespace>
        <oboInOwl:id>GAZ:00267751</oboInOwl:id>
        <rdfs:label>Reserva de la cordillera de Talamanca</rdfs:label>
    </owl:NamedIndividual>
    


    <!-- 
    ///////////////////////////////////////////////////////////////////////////////////////
    //
    // Annotations
    //
    ///////////////////////////////////////////////////////////////////////////////////////
     -->

    <rdf:Description rdf:about="http://purl.obolibrary.org/obo/GAZ_00003204">
        <oboInOwl:hasOBONamespace>GAZ</oboInOwl:hasOBONamespace>
        <oboInOwl:id>GAZ:00003204</oboInOwl:id>
        <rdfs:label>Province (Costa Rica)</rdfs:label>
    </rdf:Description>
    <rdf:Description rdf:about="http://purl.obolibrary.org/obo/GAZ_00003205">
        <oboInOwl:hasOBONamespace>GAZ</oboInOwl:hasOBONamespace>
        <rdfs:label>Alajuela Province</rdfs:label>
        <obo:IAO_0000115>A province of Costa Rica. It is located in the north-central part of the country, bordering Nicaragua to the north, and clockwise the provinces Heredia, San Jose, Puntarenas and Guanacaste. The capital is Alajuela.</obo:IAO_0000115>
        <oboInOwl:id>GAZ:00003205</oboInOwl:id>
    </rdf:Description>
    <rdf:Description rdf:about="http://purl.obolibrary.org/obo/GAZ_00003206">
        <obo:IAO_0000115>A province of Costa Rica. It is located in the eastern part of the country at the coast of the Atlantic Ocean. It borders from the south clockwise the country Panama, the provinces Puntarenas, San Jose, Cartago and Heredia, and the country Nicaragua. The capital is Limnn.</obo:IAO_0000115>
        <oboInOwl:hasOBONamespace>GAZ</oboInOwl:hasOBONamespace>
        <rdfs:label>Limon Province</rdfs:label>
        <oboInOwl:id>GAZ:00003206</oboInOwl:id>
    </rdf:Description>
    <rdf:Description rdf:about="http://purl.obolibrary.org/obo/GAZ_00003207">
        <rdfs:label>San Jose Province</rdfs:label>
        <oboInOwl:hasOBONamespace>GAZ</oboInOwl:hasOBONamespace>
        <oboInOwl:id>GAZ:00003207</oboInOwl:id>
    </rdf:Description>
    <rdf:Description rdf:about="http://purl.obolibrary.org/obo/GAZ_00003208">
        <obo:IAO_0000115>A province of Costa Rica. It is located in the north-central part of the country. To the north it borders Nicaragua, to the east is the province Limon, to the south the province San Jose, and to the west Alajuela. The capital is the city of Heredia.</obo:IAO_0000115>
        <rdfs:label>Heredia Province</rdfs:label>
        <oboInOwl:hasOBONamespace>GAZ</oboInOwl:hasOBONamespace>
        <oboInOwl:id>GAZ:00003208</oboInOwl:id>
    </rdf:Description>
    <rdf:Description rdf:about="http://purl.obolibrary.org/obo/GAZ_00003209">
        <obo:IAO_0000115>A province of Costa Rica. It is located in the western part of the country, covering most of Costa Rica&apos;s Pacific Ocean coast, and it is the largest province in Costa Rica. Clockwise from the northwest it borders on the provinces Guanacaste, Alajuela, San Jose and Limon, and the neighbouring country of Panama.</obo:IAO_0000115>
        <rdfs:label>Puntarenas Province</rdfs:label>
        <oboInOwl:hasOBONamespace>GAZ</oboInOwl:hasOBONamespace>
        <oboInOwl:id>GAZ:00003209</oboInOwl:id>
    </rdf:Description>
    <rdf:Description rdf:about="http://purl.obolibrary.org/obo/GAZ_00003210">
        <oboInOwl:id>GAZ:00003210</oboInOwl:id>
        <rdfs:label>Guanacaste Province</rdfs:label>
        <obo:IAO_0000115>A province of Costa Rica. Guanacaste is located in the northwestern part of the country, along the coast of the Pacific Ocean. To the north it borders Nicaragua. To the east is the Alajuela Province, and to the southeast is the Puntarenas Province. Guanacaste&apos;s capital is Liberia.</obo:IAO_0000115>
        <oboInOwl:hasOBONamespace>GAZ</oboInOwl:hasOBONamespace>
    </rdf:Description>
    <rdf:Description rdf:about="http://purl.obolibrary.org/obo/GAZ_00003211">
        <rdfs:label>Cartago Province</rdfs:label>
        <oboInOwl:id>GAZ:00003211</oboInOwl:id>
        <obo:IAO_0000115>A province of Costa Rica. It is located in the central part of the country. Bordering provinces are Limon to the east and San Jose to the west. The capital is Cartago.</obo:IAO_0000115>
        <oboInOwl:hasOBONamespace>GAZ</oboInOwl:hasOBONamespace>
    </rdf:Description>
    <rdf:Description rdf:about="http://purl.obolibrary.org/obo/GAZ_00007370">
        <rdfs:label>populated place, Costa Rica</rdfs:label>
        <oboInOwl:hasOBONamespace>GAZ</oboInOwl:hasOBONamespace>
        <oboInOwl:id>GAZ:00007370</oboInOwl:id>
    </rdf:Description>
    <rdf:Description rdf:about="http://purl.obolibrary.org/obo/GAZ_00007745">
        <rdfs:label>San Jose</rdfs:label>
        <obo:IAO_0000115>The capital and largest city of Costa Rica. Located in the center of the country, sprawling across the Central Valley.</obo:IAO_0000115>
        <oboInOwl:hasOBONamespace>GAZ</oboInOwl:hasOBONamespace>
        <oboInOwl:id>GAZ:00007745</oboInOwl:id>
    </rdf:Description>
    <rdf:Description rdf:about="http://purl.obolibrary.org/obo/GAZ_00007819">
        <oboInOwl:hasOBONamespace>GAZ</oboInOwl:hasOBONamespace>
        <oboInOwl:id>GAZ:00007819</oboInOwl:id>
        <rdfs:label>Golfito</rdfs:label>
    </rdf:Description>
    <rdf:Description rdf:about="http://purl.obolibrary.org/obo/GAZ_00008824">
        <obo:IAO_0000115>A populated place.</obo:IAO_0000115>
        <rdfs:label>San Isidro</rdfs:label>
        <oboInOwl:hasOBONamespace>GAZ</oboInOwl:hasOBONamespace>
        <oboInOwl:id>GAZ:00008824</oboInOwl:id>
    </rdf:Description>
</rdf:RDF>



<!-- Generated by the OWL API (version 4.5.6) https://github.com/owlcs/owlapi -->

