<?xml version="1.0"?>
<rdf:RDF xmlns="http://purl.obolibrary.org/obo/gaz/subsets/countries/Djibouti.owl#"
     xml:base="http://purl.obolibrary.org/obo/gaz/subsets/countries/Djibouti.owl"
     xmlns:obo="http://purl.obolibrary.org/obo/"
     xmlns:owl="http://www.w3.org/2002/07/owl#"
     xmlns:rdf="http://www.w3.org/1999/02/22-rdf-syntax-ns#"
     xmlns:xml="http://www.w3.org/XML/1998/namespace"
     xmlns:xsd="http://www.w3.org/2001/XMLSchema#"
     xmlns:rdfs="http://www.w3.org/2000/01/rdf-schema#"
     xmlns:oboInOwl="http://www.geneontology.org/formats/oboInOwl#">
    <owl:Ontology rdf:about="http://purl.obolibrary.org/obo/gaz/subsets/countries/Djibouti.owl">
        <owl:imports rdf:resource="http://purl.obolibrary.org/obo/gaz/imports/envo_import.owl"/>
        <owl:imports rdf:resource="http://purl.obolibrary.org/obo/gaz/imports/ro_import.owl"/>
    </owl:Ontology>
    


    <!-- 
    ///////////////////////////////////////////////////////////////////////////////////////
    //
    // Annotation properties
    //
    ///////////////////////////////////////////////////////////////////////////////////////
     -->

    


    <!-- http://purl.obolibrary.org/obo/IAO_0000115 -->

    <owl:AnnotationProperty rdf:about="http://purl.obolibrary.org/obo/IAO_0000115"/>
    


    <!-- http://www.geneontology.org/formats/oboInOwl#hasOBONamespace -->

    <owl:AnnotationProperty rdf:about="http://www.geneontology.org/formats/oboInOwl#hasOBONamespace"/>
    


    <!-- http://www.geneontology.org/formats/oboInOwl#id -->

    <owl:AnnotationProperty rdf:about="http://www.geneontology.org/formats/oboInOwl#id"/>
    


    <!-- 
    ///////////////////////////////////////////////////////////////////////////////////////
    //
    // Object Properties
    //
    ///////////////////////////////////////////////////////////////////////////////////////
     -->

    


    <!-- http://purl.obolibrary.org/obo/RO_0001025 -->

    <owl:ObjectProperty rdf:about="http://purl.obolibrary.org/obo/RO_0001025"/>
    


    <!-- 
    ///////////////////////////////////////////////////////////////////////////////////////
    //
    // Classes
    //
    ///////////////////////////////////////////////////////////////////////////////////////
     -->

    


    <!-- http://purl.obolibrary.org/obo/ENVO_00000009 -->

    <owl:Class rdf:about="http://purl.obolibrary.org/obo/ENVO_00000009"/>
    


    <!-- http://purl.obolibrary.org/obo/ENVO_00000354 -->

    <owl:Class rdf:about="http://purl.obolibrary.org/obo/ENVO_00000354"/>
    


    <!-- http://purl.obolibrary.org/obo/GAZ_00000790 -->

    <owl:Class rdf:about="http://purl.obolibrary.org/obo/GAZ_00000790"/>
    


    <!-- http://purl.obolibrary.org/obo/GAZ_00000791 -->

    <owl:Class rdf:about="http://purl.obolibrary.org/obo/GAZ_00000791">
        <rdfs:subClassOf rdf:resource="http://purl.obolibrary.org/obo/GAZ_00000790"/>
        <obo:IAO_0000115>A region in Djibouti. Its capital is Ali Sabieh. Other major cities and towns include Holhol. Ali Sabieh borders Arta Region to the north, Somaliland (Somalia) to the east, Ethiopia to the south and the Dikhil Region to the west.</obo:IAO_0000115>
        <oboInOwl:hasOBONamespace>GAZ</oboInOwl:hasOBONamespace>
        <oboInOwl:id>GAZ:00000791</oboInOwl:id>
        <rdfs:label>Ali Sabieh Region</rdfs:label>
    </owl:Class>
    


    <!-- http://purl.obolibrary.org/obo/GAZ_00000792 -->

    <owl:Class rdf:about="http://purl.obolibrary.org/obo/GAZ_00000792">
        <rdfs:subClassOf rdf:resource="http://purl.obolibrary.org/obo/GAZ_00000790"/>
    </owl:Class>
    


    <!-- http://purl.obolibrary.org/obo/GAZ_00000793 -->

    <owl:Class rdf:about="http://purl.obolibrary.org/obo/GAZ_00000793">
        <rdfs:subClassOf rdf:resource="http://purl.obolibrary.org/obo/GAZ_00000790"/>
    </owl:Class>
    


    <!-- http://purl.obolibrary.org/obo/GAZ_00000794 -->

    <owl:Class rdf:about="http://purl.obolibrary.org/obo/GAZ_00000794">
        <rdfs:subClassOf rdf:resource="http://purl.obolibrary.org/obo/GAZ_00001011"/>
        <rdfs:subClassOf rdf:resource="http://purl.obolibrary.org/obo/GAZ_00008577"/>
    </owl:Class>
    


    <!-- http://purl.obolibrary.org/obo/GAZ_00000795 -->

    <owl:Class rdf:about="http://purl.obolibrary.org/obo/GAZ_00000795">
        <rdfs:subClassOf rdf:resource="http://purl.obolibrary.org/obo/GAZ_00000790"/>
    </owl:Class>
    


    <!-- http://purl.obolibrary.org/obo/GAZ_00000796 -->

    <owl:Class rdf:about="http://purl.obolibrary.org/obo/GAZ_00000796">
        <rdfs:subClassOf rdf:resource="http://purl.obolibrary.org/obo/GAZ_00000790"/>
    </owl:Class>
    


    <!-- http://purl.obolibrary.org/obo/GAZ_00001011 -->

    <owl:Class rdf:about="http://purl.obolibrary.org/obo/GAZ_00001011"/>
    


    <!-- http://purl.obolibrary.org/obo/GAZ_00008576 -->

    <owl:Class rdf:about="http://purl.obolibrary.org/obo/GAZ_00008576">
        <rdfs:subClassOf rdf:resource="http://purl.obolibrary.org/obo/GAZ_00008577"/>
    </owl:Class>
    


    <!-- http://purl.obolibrary.org/obo/GAZ_00008577 -->

    <owl:Class rdf:about="http://purl.obolibrary.org/obo/GAZ_00008577"/>
    


    <!-- 
    ///////////////////////////////////////////////////////////////////////////////////////
    //
    // Individuals
    //
    ///////////////////////////////////////////////////////////////////////////////////////
     -->

    


    <!-- http://purl.obolibrary.org/obo/GAZ_00000582 -->

    <owl:NamedIndividual rdf:about="http://purl.obolibrary.org/obo/GAZ_00000582">
        <rdf:type rdf:resource="http://purl.obolibrary.org/obo/ENVO_00000009"/>
        <obo:IAO_0000115>A country in eastern Africa. Djibouti is bordered by Eritrea in the north, Ethiopia in the west and south, and Somalia in the southeast. The remainder of the border is formed by the Red Sea and the Gulf of Aden. On the other side of the Red Sea, on the Arabian Peninsula, 20 km from the coast of Djibouti, is Yemen. The capital of Djibouti is the city of Djibouti. Djibouti is divided into 5 regions and one city. It is further subdivided into 11 districts.</obo:IAO_0000115>
        <oboInOwl:hasOBONamespace>GAZ</oboInOwl:hasOBONamespace>
        <oboInOwl:id>GAZ:00000582</oboInOwl:id>
        <rdfs:label>Djibouti</rdfs:label>
    </owl:NamedIndividual>
    


    <!-- http://purl.obolibrary.org/obo/GAZ_00000790 -->

    <owl:NamedIndividual rdf:about="http://purl.obolibrary.org/obo/GAZ_00000790">
        <obo:RO_0001025 rdf:resource="http://purl.obolibrary.org/obo/GAZ_00000582"/>
    </owl:NamedIndividual>
    


    <!-- http://purl.obolibrary.org/obo/GAZ_00000792 -->

    <owl:NamedIndividual rdf:about="http://purl.obolibrary.org/obo/GAZ_00000792"/>
    


    <!-- http://purl.obolibrary.org/obo/GAZ_00000793 -->

    <owl:NamedIndividual rdf:about="http://purl.obolibrary.org/obo/GAZ_00000793"/>
    


    <!-- http://purl.obolibrary.org/obo/GAZ_00000794 -->

    <owl:NamedIndividual rdf:about="http://purl.obolibrary.org/obo/GAZ_00000794"/>
    


    <!-- http://purl.obolibrary.org/obo/GAZ_00000795 -->

    <owl:NamedIndividual rdf:about="http://purl.obolibrary.org/obo/GAZ_00000795"/>
    


    <!-- http://purl.obolibrary.org/obo/GAZ_00000796 -->

    <owl:NamedIndividual rdf:about="http://purl.obolibrary.org/obo/GAZ_00000796"/>
    


    <!-- http://purl.obolibrary.org/obo/GAZ_00001011 -->

    <owl:NamedIndividual rdf:about="http://purl.obolibrary.org/obo/GAZ_00001011">
        <obo:RO_0001025 rdf:resource="http://purl.obolibrary.org/obo/GAZ_00000582"/>
    </owl:NamedIndividual>
    


    <!-- http://purl.obolibrary.org/obo/GAZ_00008576 -->

    <owl:NamedIndividual rdf:about="http://purl.obolibrary.org/obo/GAZ_00008576">
        <obo:RO_0001025 rdf:resource="http://purl.obolibrary.org/obo/GAZ_02000475"/>
    </owl:NamedIndividual>
    


    <!-- http://purl.obolibrary.org/obo/GAZ_00008577 -->

    <owl:NamedIndividual rdf:about="http://purl.obolibrary.org/obo/GAZ_00008577">
        <obo:RO_0001025 rdf:resource="http://purl.obolibrary.org/obo/GAZ_00000582"/>
    </owl:NamedIndividual>
    


    <!-- http://purl.obolibrary.org/obo/GAZ_00039902 -->

    <owl:NamedIndividual rdf:about="http://purl.obolibrary.org/obo/GAZ_00039902">
        <obo:RO_0001025 rdf:resource="http://purl.obolibrary.org/obo/GAZ_00000795"/>
        <obo:IAO_0000115>A group of small islands off of the eastern coast of the Horn of Africa, in the Dact-el-Mayun section of the Bab-el-Mandeb strait.</obo:IAO_0000115>
        <oboInOwl:hasOBONamespace>GAZ</oboInOwl:hasOBONamespace>
        <oboInOwl:id>GAZ:00039902</oboInOwl:id>
        <rdfs:label>Sept Freres</rdfs:label>
    </owl:NamedIndividual>
    


    <!-- http://purl.obolibrary.org/obo/GAZ_00039903 -->

    <owl:NamedIndividual rdf:about="http://purl.obolibrary.org/obo/GAZ_00039903">
        <obo:RO_0001025 rdf:resource="http://purl.obolibrary.org/obo/GAZ_00000794"/>
        <obo:RO_0001025 rdf:resource="http://purl.obolibrary.org/obo/GAZ_00052528"/>
        <obo:IAO_0000115>A small coral island of Djibouti, at the center of the Gulf of Tadjoura.</obo:IAO_0000115>
        <oboInOwl:hasOBONamespace>GAZ</oboInOwl:hasOBONamespace>
        <oboInOwl:id>GAZ:00039903</oboInOwl:id>
        <rdfs:label>Ile Moucha</rdfs:label>
    </owl:NamedIndividual>
    


    <!-- http://purl.obolibrary.org/obo/GAZ_00039904 -->

    <owl:NamedIndividual rdf:about="http://purl.obolibrary.org/obo/GAZ_00039904">
        <obo:RO_0001025 rdf:resource="http://purl.obolibrary.org/obo/GAZ_00000794"/>
        <obo:RO_0001025 rdf:resource="http://purl.obolibrary.org/obo/GAZ_00052528"/>
        <obo:IAO_0000115>A small island near Moucha Island in the Gulf of Tadjoura.</obo:IAO_0000115>
        <oboInOwl:hasOBONamespace>GAZ</oboInOwl:hasOBONamespace>
        <oboInOwl:id>GAZ:00039904</oboInOwl:id>
        <rdfs:label>Ile Maskali</rdfs:label>
    </owl:NamedIndividual>
    


    <!-- http://purl.obolibrary.org/obo/GAZ_00052528 -->

    <owl:NamedIndividual rdf:about="http://purl.obolibrary.org/obo/GAZ_00052528">
        <obo:IAO_0000115>A gulf or basin of the Indian Ocean in the Horn of Africa, lying to the south of the straits of Bab-el-Mandeb, or the entrance to the Red Sea. Most of its coastline is the territory of Djibouti, except for a short stretch on the southern shore which is part of the territory of Somalia. Ports on the Gulf of Tadjoura include Obock, Tadjoura and Djibouti City.</obo:IAO_0000115>
        <oboInOwl:hasOBONamespace>GAZ</oboInOwl:hasOBONamespace>
        <oboInOwl:id>GAZ:00052528</oboInOwl:id>
        <rdfs:label>Gulf of Tadjoura</rdfs:label>
    </owl:NamedIndividual>
    


    <!-- http://purl.obolibrary.org/obo/GAZ_00052684 -->

    <owl:NamedIndividual rdf:about="http://purl.obolibrary.org/obo/GAZ_00052684">
        <obo:RO_0001025 rdf:resource="http://purl.obolibrary.org/obo/GAZ_00000796"/>
        <obo:IAO_0000115>A saline crater lake in central Djibouti, located at the southern border of Tadjoura Region, touching Dikhil Region. Fed by subterranean inflows which include infiltration of sea water, as well as by wadis which lead into the depression.</obo:IAO_0000115>
        <oboInOwl:hasOBONamespace>GAZ</oboInOwl:hasOBONamespace>
        <oboInOwl:id>GAZ:00052684</oboInOwl:id>
        <rdfs:label>Lake Asal</rdfs:label>
    </owl:NamedIndividual>
    


    <!-- http://purl.obolibrary.org/obo/GAZ_00052685 -->

    <owl:NamedIndividual rdf:about="http://purl.obolibrary.org/obo/GAZ_00052685">
        <obo:RO_0001025 rdf:resource="http://purl.obolibrary.org/obo/GAZ_00000796"/>
        <obo:IAO_0000115>A national park in Djibouti.</obo:IAO_0000115>
        <oboInOwl:hasOBONamespace>GAZ</oboInOwl:hasOBONamespace>
        <oboInOwl:id>GAZ:00052685</oboInOwl:id>
        <rdfs:label>Day Forest National Park</rdfs:label>
    </owl:NamedIndividual>
    


    <!-- http://purl.obolibrary.org/obo/GAZ_00053633 -->

    <owl:NamedIndividual rdf:about="http://purl.obolibrary.org/obo/GAZ_00053633">
        <obo:RO_0001025 rdf:resource="http://purl.obolibrary.org/obo/GAZ_00000582"/>
        <obo:IAO_0000115>A series of NW-trending fissure vents and pyroclastic cones along the Ethiopia-Djibouti border. The elongated complex represents an uplifted mid-ocean ridge spreading center now exposed above sea level. An elongated dome of basement rocks is cut by two axial rifts, the northern of which was active during historical time. Basaltic cinder cones along marginal faults of the rift have produced lava flows that traveled down the flanks of the structural dome, producing a shield-like morphology.</obo:IAO_0000115>
        <oboInOwl:hasOBONamespace>GAZ</oboInOwl:hasOBONamespace>
        <oboInOwl:id>GAZ:00053633</oboInOwl:id>
        <rdfs:label>Manda-Inakir</rdfs:label>
    </owl:NamedIndividual>
    


    <!-- http://purl.obolibrary.org/obo/GAZ_00053634 -->

    <owl:NamedIndividual rdf:about="http://purl.obolibrary.org/obo/GAZ_00053634">
        <obo:RO_0001025 rdf:resource="http://purl.obolibrary.org/obo/GAZ_00053633"/>
        <obo:IAO_0000115>A cinder cone.</obo:IAO_0000115>
        <oboInOwl:hasOBONamespace>GAZ</oboInOwl:hasOBONamespace>
        <oboInOwl:id>GAZ:00053634</oboInOwl:id>
        <rdfs:label>Kammourta</rdfs:label>
    </owl:NamedIndividual>
    


    <!-- http://purl.obolibrary.org/obo/GAZ_00053635 -->

    <owl:NamedIndividual rdf:about="http://purl.obolibrary.org/obo/GAZ_00053635">
        <rdf:type rdf:resource="http://purl.obolibrary.org/obo/ENVO_00000354"/>
        <obo:RO_0001025 rdf:resource="http://purl.obolibrary.org/obo/GAZ_00000796"/>
        <obo:IAO_0000115>A volcanic complex that is a large Holocene stratovolcano constructed along the border between Ethiopia, Eritrea, and Djibouti. The 2028 m high trachytic-to-rhyolitic volcano is the most prominent topographic feature in this area and towers above its neighbor to the SW, Manda Inakir. Rhyolitic lava domes and lava flows are found in the summit region, which is truncated by a caldera.</obo:IAO_0000115>
        <oboInOwl:hasOBONamespace>GAZ</oboInOwl:hasOBONamespace>
        <oboInOwl:id>GAZ:00053635</oboInOwl:id>
        <rdfs:label>Mousa Alli Volcanic Complex</rdfs:label>
    </owl:NamedIndividual>
    


    <!-- http://purl.obolibrary.org/obo/GAZ_00053636 -->

    <owl:NamedIndividual rdf:about="http://purl.obolibrary.org/obo/GAZ_00053636">
        <obo:RO_0001025 rdf:resource="http://purl.obolibrary.org/obo/GAZ_00000582"/>
        <obo:IAO_0000115>A volcanic field, located along the Eritrea/Djibouti border, consists of a group of basaltic scoria cones and lava flows aligned in an E-W direction NE of the large Mousa Alli stratovolcano. A second E-W-trending chain of cones is located to the north of the principal chain, most of which lies in Eritrea, and fed long lava flows that descend to the north, in the direction of the Red Sea.</obo:IAO_0000115>
        <oboInOwl:hasOBONamespace>GAZ</oboInOwl:hasOBONamespace>
        <oboInOwl:id>GAZ:00053636</oboInOwl:id>
        <rdfs:label>Gufa Volcanic Field</rdfs:label>
    </owl:NamedIndividual>
    


    <!-- http://purl.obolibrary.org/obo/GAZ_00053638 -->

    <owl:NamedIndividual rdf:about="http://purl.obolibrary.org/obo/GAZ_00053638">
        <obo:RO_0001025 rdf:resource="http://purl.obolibrary.org/obo/GAZ_00000796"/>
        <obo:IAO_0000115>Fissure vents trending NW from the Red Sea, contains a broad area of youthful fissure vents between Lake Asal and the Ghoubbat al Kharab gulf. The rift is subaerially exposed over a 12 km distance between these two bodies of water and contains numerous basaltic cinder and spatter cones. Magma-water interaction has produced tuff cones, some of which form islands or are breached by the sea. The most recent lava flows are younger than lake sediments deposited 5300 years ago.</obo:IAO_0000115>
        <oboInOwl:hasOBONamespace>GAZ</oboInOwl:hasOBONamespace>
        <oboInOwl:id>GAZ:00053638</oboInOwl:id>
        <rdfs:label>Ardoukoba Rift</rdfs:label>
    </owl:NamedIndividual>
    


    <!-- http://purl.obolibrary.org/obo/GAZ_00053639 -->

    <owl:NamedIndividual rdf:about="http://purl.obolibrary.org/obo/GAZ_00053639">
        <obo:RO_0001025 rdf:resource="http://purl.obolibrary.org/obo/GAZ_00000582"/>
        <obo:IAO_0000115>A fumarole field near the SE end of the Hanleh Plain is located along an escarpment in an area of Plio-Pleistocene basaltic volcanic rocks.</obo:IAO_0000115>
        <oboInOwl:hasOBONamespace>GAZ</oboInOwl:hasOBONamespace>
        <oboInOwl:id>GAZ:00053639</oboInOwl:id>
        <rdfs:label>Garbes Fumarole Field</rdfs:label>
    </owl:NamedIndividual>
    


    <!-- http://purl.obolibrary.org/obo/GAZ_00053640 -->

    <owl:NamedIndividual rdf:about="http://purl.obolibrary.org/obo/GAZ_00053640">
        <obo:RO_0001025 rdf:resource="http://purl.obolibrary.org/obo/GAZ_00000582"/>
        <obo:IAO_0000115>A fumarole field immediately north of Lake Abbe. The fumaroles are located in a 7-m-deep funnel about 300 m above the surface of Lake Abbe and about 1 km NE of its shore; they are visible and audible from a distance.</obo:IAO_0000115>
        <oboInOwl:hasOBONamespace>GAZ</oboInOwl:hasOBONamespace>
        <oboInOwl:id>GAZ:00053640</oboInOwl:id>
        <rdfs:label>Boina Fumurole Field</rdfs:label>
    </owl:NamedIndividual>
    


    <!-- http://purl.obolibrary.org/obo/GAZ_00057510 -->

    <owl:NamedIndividual rdf:about="http://purl.obolibrary.org/obo/GAZ_00057510">
        <obo:IAO_0000115>An endorheic saline lake lying on the Ethiopia-Djibouti border, and is one of a chain of six connected lakes which also includes (from north to south) lakes Gargori, Laitali, Gummare, Bario and Afambo. Lake Abbe is the ultimate destination of the waters of the Awash River. Lake Abbe is at the central point of the Afar Depression, where three pieces of the earth&apos;s crust meet. On the northwest shore rises Dama Ali, a volcanic mountain.</obo:IAO_0000115>
        <oboInOwl:hasOBONamespace>GAZ</oboInOwl:hasOBONamespace>
        <oboInOwl:id>GAZ:00057510</oboInOwl:id>
        <rdfs:label>Lake Abbe</rdfs:label>
    </owl:NamedIndividual>
    


    <!-- http://purl.obolibrary.org/obo/GAZ_00076347 -->

    <owl:NamedIndividual rdf:about="http://purl.obolibrary.org/obo/GAZ_00076347">
        <obo:RO_0001025 rdf:resource="http://purl.obolibrary.org/obo/GAZ_00000582"/>
        <obo:IAO_0000115>A national park in Dijuti.</obo:IAO_0000115>
        <oboInOwl:hasOBONamespace>GAZ</oboInOwl:hasOBONamespace>
        <oboInOwl:id>GAZ:00076347</oboInOwl:id>
        <rdfs:label>Djibouti National Park</rdfs:label>
    </owl:NamedIndividual>
    


    <!-- http://purl.obolibrary.org/obo/GAZ_00076348 -->

    <owl:NamedIndividual rdf:about="http://purl.obolibrary.org/obo/GAZ_00076348">
        <obo:RO_0001025 rdf:resource="http://purl.obolibrary.org/obo/GAZ_00000793"/>
        <obo:IAO_0000115>A national park in Djibuti.</obo:IAO_0000115>
        <oboInOwl:hasOBONamespace>GAZ</oboInOwl:hasOBONamespace>
        <oboInOwl:id>GAZ:00076348</oboInOwl:id>
        <rdfs:label>Yoboki National Park</rdfs:label>
    </owl:NamedIndividual>
    


    <!-- http://purl.obolibrary.org/obo/GAZ_00076353 -->

    <owl:NamedIndividual rdf:about="http://purl.obolibrary.org/obo/GAZ_00076353">
        <obo:RO_0001025 rdf:resource="http://purl.obolibrary.org/obo/GAZ_00000792"/>
        <oboInOwl:hasOBONamespace>GAZ</oboInOwl:hasOBONamespace>
        <oboInOwl:id>GAZ:00076353</oboInOwl:id>
        <rdfs:label>Arta District</rdfs:label>
    </owl:NamedIndividual>
    


    <!-- http://purl.obolibrary.org/obo/GAZ_00076354 -->

    <owl:NamedIndividual rdf:about="http://purl.obolibrary.org/obo/GAZ_00076354">
        <obo:RO_0001025 rdf:resource="http://purl.obolibrary.org/obo/GAZ_00000794"/>
        <oboInOwl:hasOBONamespace>GAZ</oboInOwl:hasOBONamespace>
        <oboInOwl:id>GAZ:00076354</oboInOwl:id>
        <rdfs:label>1er arrondissement</rdfs:label>
    </owl:NamedIndividual>
    


    <!-- http://purl.obolibrary.org/obo/GAZ_00076355 -->

    <owl:NamedIndividual rdf:about="http://purl.obolibrary.org/obo/GAZ_00076355">
        <obo:RO_0001025 rdf:resource="http://purl.obolibrary.org/obo/GAZ_00000794"/>
        <oboInOwl:hasOBONamespace>GAZ</oboInOwl:hasOBONamespace>
        <oboInOwl:id>GAZ:00076355</oboInOwl:id>
        <rdfs:label>2e arrondissement</rdfs:label>
    </owl:NamedIndividual>
    


    <!-- http://purl.obolibrary.org/obo/GAZ_00076356 -->

    <owl:NamedIndividual rdf:about="http://purl.obolibrary.org/obo/GAZ_00076356">
        <obo:RO_0001025 rdf:resource="http://purl.obolibrary.org/obo/GAZ_00000794"/>
        <oboInOwl:hasOBONamespace>GAZ</oboInOwl:hasOBONamespace>
        <oboInOwl:id>GAZ:00076356</oboInOwl:id>
        <rdfs:label>5e arrondissement</rdfs:label>
    </owl:NamedIndividual>
    


    <!-- http://purl.obolibrary.org/obo/GAZ_00076357 -->

    <owl:NamedIndividual rdf:about="http://purl.obolibrary.org/obo/GAZ_00076357">
        <obo:RO_0001025 rdf:resource="http://purl.obolibrary.org/obo/GAZ_00000794"/>
        <oboInOwl:hasOBONamespace>GAZ</oboInOwl:hasOBONamespace>
        <oboInOwl:id>GAZ:00076357</oboInOwl:id>
        <rdfs:label>4e arrondissement</rdfs:label>
    </owl:NamedIndividual>
    


    <!-- http://purl.obolibrary.org/obo/GAZ_00076358 -->

    <owl:NamedIndividual rdf:about="http://purl.obolibrary.org/obo/GAZ_00076358">
        <obo:RO_0001025 rdf:resource="http://purl.obolibrary.org/obo/GAZ_00000794"/>
        <oboInOwl:hasOBONamespace>GAZ</oboInOwl:hasOBONamespace>
        <oboInOwl:id>GAZ:00076358</oboInOwl:id>
        <rdfs:label>3e arrondissement</rdfs:label>
    </owl:NamedIndividual>
    


    <!-- http://purl.obolibrary.org/obo/GAZ_00102119 -->

    <owl:NamedIndividual rdf:about="http://purl.obolibrary.org/obo/GAZ_00102119">
        <obo:RO_0001025 rdf:resource="http://purl.obolibrary.org/obo/GAZ_00000796"/>
        <obo:IAO_0000115>Mountains that lie north west of the Gulf of Tadjoura in Djibouti. Part of the mountains is protected as the Day Forest National Park.</obo:IAO_0000115>
        <oboInOwl:hasOBONamespace>GAZ</oboInOwl:hasOBONamespace>
        <oboInOwl:id>GAZ:00102119</oboInOwl:id>
        <rdfs:label>Goda Mountains</rdfs:label>
    </owl:NamedIndividual>
    


    <!-- http://purl.obolibrary.org/obo/GAZ_00102120 -->

    <owl:NamedIndividual rdf:about="http://purl.obolibrary.org/obo/GAZ_00102120">
        <obo:RO_0001025 rdf:resource="http://purl.obolibrary.org/obo/GAZ_00000795"/>
        <obo:IAO_0000115>A peninsula in Obock Region, Djibouti.</obo:IAO_0000115>
        <oboInOwl:hasOBONamespace>GAZ</oboInOwl:hasOBONamespace>
        <oboInOwl:id>GAZ:00102120</oboInOwl:id>
        <rdfs:label>Ras Siyan</rdfs:label>
    </owl:NamedIndividual>
    


    <!-- http://purl.obolibrary.org/obo/GAZ_00241986 -->

    <owl:NamedIndividual rdf:about="http://purl.obolibrary.org/obo/GAZ_00241986">
        <obo:RO_0001025 rdf:resource="http://purl.obolibrary.org/obo/GAZ_00000794"/>
        <obo:RO_0001025 rdf:resource="http://purl.obolibrary.org/obo/GAZ_00052528"/>
        <obo:IAO_0000115>An island.</obo:IAO_0000115>
        <oboInOwl:hasOBONamespace>GAZ</oboInOwl:hasOBONamespace>
        <oboInOwl:id>GAZ:00241986</oboInOwl:id>
        <rdfs:label>Ile de Ouaramous</rdfs:label>
    </owl:NamedIndividual>
    


    <!-- http://purl.obolibrary.org/obo/GAZ_02000475 -->

    <owl:NamedIndividual rdf:about="http://purl.obolibrary.org/obo/GAZ_02000475">
        <obo:RO_0001025 rdf:resource="http://purl.obolibrary.org/obo/GAZ_00000795"/>
        <obo:IAO_0000115>A District of Djibouti.</obo:IAO_0000115>
        <oboInOwl:hasOBONamespace>GAZ</oboInOwl:hasOBONamespace>
        <oboInOwl:id>GAZ:02000475</oboInOwl:id>
        <rdfs:label>Obock District</rdfs:label>
    </owl:NamedIndividual>
    


    <!-- http://purl.obolibrary.org/obo/GAZ_02000476 -->

    <owl:NamedIndividual rdf:about="http://purl.obolibrary.org/obo/GAZ_02000476">
        <obo:RO_0001025 rdf:resource="http://purl.obolibrary.org/obo/GAZ_00000795"/>
        <obo:IAO_0000115>A District of Djibouti.</obo:IAO_0000115>
        <oboInOwl:hasOBONamespace>GAZ</oboInOwl:hasOBONamespace>
        <oboInOwl:id>GAZ:02000476</oboInOwl:id>
        <rdfs:label>Alaili Dadda District</rdfs:label>
    </owl:NamedIndividual>
    


    <!-- http://purl.obolibrary.org/obo/GAZ_02000477 -->

    <owl:NamedIndividual rdf:about="http://purl.obolibrary.org/obo/GAZ_02000477">
        <obo:RO_0001025 rdf:resource="http://purl.obolibrary.org/obo/GAZ_00000796"/>
        <obo:IAO_0000115>A District of Djibouti.</obo:IAO_0000115>
        <oboInOwl:hasOBONamespace>GAZ</oboInOwl:hasOBONamespace>
        <oboInOwl:id>GAZ:02000477</oboInOwl:id>
        <rdfs:label>Tadjourah District</rdfs:label>
    </owl:NamedIndividual>
    


    <!-- http://purl.obolibrary.org/obo/GAZ_02000478 -->

    <owl:NamedIndividual rdf:about="http://purl.obolibrary.org/obo/GAZ_02000478">
        <obo:RO_0001025 rdf:resource="http://purl.obolibrary.org/obo/GAZ_00000796"/>
        <obo:IAO_0000115>A District of Djibouti.</obo:IAO_0000115>
        <oboInOwl:hasOBONamespace>GAZ</oboInOwl:hasOBONamespace>
        <oboInOwl:id>GAZ:02000478</oboInOwl:id>
        <rdfs:label>Randa District</rdfs:label>
    </owl:NamedIndividual>
    


    <!-- http://purl.obolibrary.org/obo/GAZ_02000479 -->

    <owl:NamedIndividual rdf:about="http://purl.obolibrary.org/obo/GAZ_02000479">
        <obo:RO_0001025 rdf:resource="http://purl.obolibrary.org/obo/GAZ_00000796"/>
        <obo:IAO_0000115>A District of Djibouti.</obo:IAO_0000115>
        <oboInOwl:hasOBONamespace>GAZ</oboInOwl:hasOBONamespace>
        <oboInOwl:id>GAZ:02000479</oboInOwl:id>
        <rdfs:label>Dorra District</rdfs:label>
    </owl:NamedIndividual>
    


    <!-- http://purl.obolibrary.org/obo/GAZ_02000480 -->

    <owl:NamedIndividual rdf:about="http://purl.obolibrary.org/obo/GAZ_02000480">
        <obo:RO_0001025 rdf:resource="http://purl.obolibrary.org/obo/GAZ_00000796"/>
        <obo:IAO_0000115>A District of Djibouti.</obo:IAO_0000115>
        <oboInOwl:hasOBONamespace>GAZ</oboInOwl:hasOBONamespace>
        <oboInOwl:id>GAZ:02000480</oboInOwl:id>
        <rdfs:label>Balha District</rdfs:label>
    </owl:NamedIndividual>
    


    <!-- http://purl.obolibrary.org/obo/GAZ_02000481 -->

    <owl:NamedIndividual rdf:about="http://purl.obolibrary.org/obo/GAZ_02000481">
        <obo:RO_0001025 rdf:resource="http://purl.obolibrary.org/obo/GAZ_00000793"/>
        <obo:IAO_0000115>A District of Djibouti.</obo:IAO_0000115>
        <oboInOwl:hasOBONamespace>GAZ</oboInOwl:hasOBONamespace>
        <oboInOwl:id>GAZ:02000481</oboInOwl:id>
        <rdfs:label>As Eyla District</rdfs:label>
    </owl:NamedIndividual>
    


    <!-- 
    ///////////////////////////////////////////////////////////////////////////////////////
    //
    // Annotations
    //
    ///////////////////////////////////////////////////////////////////////////////////////
     -->

    <rdf:Description rdf:about="http://purl.obolibrary.org/obo/GAZ_00000790">
        <oboInOwl:hasOBONamespace>GAZ</oboInOwl:hasOBONamespace>
        <rdfs:label>Region (Djibouti)</rdfs:label>
        <oboInOwl:id>GAZ:00000790</oboInOwl:id>
    </rdf:Description>
    <rdf:Description rdf:about="http://purl.obolibrary.org/obo/GAZ_00000792">
        <oboInOwl:hasOBONamespace>GAZ</oboInOwl:hasOBONamespace>
        <obo:IAO_0000115>A region in Djibouti. Its capital is Arta.</obo:IAO_0000115>
        <oboInOwl:id>GAZ:00000792</oboInOwl:id>
        <rdfs:label>Arta Region</rdfs:label>
    </rdf:Description>
    <rdf:Description rdf:about="http://purl.obolibrary.org/obo/GAZ_00000793">
        <rdfs:label>Dikhil Region</rdfs:label>
        <oboInOwl:id>GAZ:00000793</oboInOwl:id>
        <obo:IAO_0000115>A region in Djibouti. Its capital is Dikhil. Other major cities and towns include As Ela, Galafi and Yoboki. The district borders Tadjourah Region to the north, Ethiopia to the west/south, the Gulf of Tadjourah to the north and Arta Region and Ali Sabieh Region to the east. The district contains part of Lake Abhe Bad, which it shares with Ethiopia.</obo:IAO_0000115>
        <oboInOwl:hasOBONamespace>GAZ</oboInOwl:hasOBONamespace>
    </rdf:Description>
    <rdf:Description rdf:about="http://purl.obolibrary.org/obo/GAZ_00000794">
        <rdfs:label>Djibouti City</rdfs:label>
        <oboInOwl:id>GAZ:00000794</oboInOwl:id>
        <obo:IAO_0000115>The capital and largest city of the Republic of Djibouti. It lies on a peninsula that divides the Gulf of Aden from the Gulf of Tadjoura. Djibouti has the same status as the country&apos;s five regions. The metropolitan territory borders Arta Region to the south and west, and the Gulf of Tadjourah/Gulf of Aden to the north.</obo:IAO_0000115>
        <oboInOwl:hasOBONamespace>GAZ</oboInOwl:hasOBONamespace>
    </rdf:Description>
    <rdf:Description rdf:about="http://purl.obolibrary.org/obo/GAZ_00000795">
        <obo:IAO_0000115>A region in Djibouti. Its capital is Obock. Other major cities and towns include Khor Angar. The district borders Eritrea to the north, Tadjourah Region to the south-west and the Red Sea/Bab el Mandeb/Gulf of Aden to the east/south-east.</obo:IAO_0000115>
        <oboInOwl:id>GAZ:00000795</oboInOwl:id>
        <oboInOwl:hasOBONamespace>GAZ</oboInOwl:hasOBONamespace>
        <rdfs:label>Obock Region</rdfs:label>
    </rdf:Description>
    <rdf:Description rdf:about="http://purl.obolibrary.org/obo/GAZ_00000796">
        <obo:IAO_0000115>A region in Djibouti. The district borders Ethiopia and Eritrea to the north/north-west, Obock Region to the north-east, Dikhil and Arta regions to the south and the Gulf of Tadjourah to the south-east. Lake Asal is located in the south of the district. The capital of Tadjourah Region is Tadjourah. Other major cities and towns include Randa, Dorra and Balha.</obo:IAO_0000115>
        <oboInOwl:hasOBONamespace>GAZ</oboInOwl:hasOBONamespace>
        <oboInOwl:id>GAZ:00000796</oboInOwl:id>
        <rdfs:label>Tadjourah Region</rdfs:label>
    </rdf:Description>
    <rdf:Description rdf:about="http://purl.obolibrary.org/obo/GAZ_00001011">
        <rdfs:label>Ville (Djibouti)</rdfs:label>
        <oboInOwl:hasOBONamespace>GAZ</oboInOwl:hasOBONamespace>
        <oboInOwl:id>GAZ:00001011</oboInOwl:id>
    </rdf:Description>
    <rdf:Description rdf:about="http://purl.obolibrary.org/obo/GAZ_00008576">
        <obo:IAO_0000115>A small port town of Djibouti, located on the northern shore of the Gulf of Tadjoura where it opens out into the Gulf of Aden.</obo:IAO_0000115>
        <oboInOwl:hasOBONamespace>GAZ</oboInOwl:hasOBONamespace>
        <rdfs:label>Obock</rdfs:label>
        <oboInOwl:id>GAZ:00008576</oboInOwl:id>
    </rdf:Description>
    <rdf:Description rdf:about="http://purl.obolibrary.org/obo/GAZ_00008577">
        <oboInOwl:hasOBONamespace>GAZ</oboInOwl:hasOBONamespace>
        <rdfs:label>populated place, Dijubti</rdfs:label>
        <oboInOwl:id>GAZ:00008577</oboInOwl:id>
    </rdf:Description>
</rdf:RDF>



<!-- Generated by the OWL API (version 4.5.6) https://github.com/owlcs/owlapi -->

