<?xml version="1.0"?>
<rdf:RDF xmlns="http://purl.obolibrary.org/obo/gaz/subsets/countries/Egypt.owl#"
     xml:base="http://purl.obolibrary.org/obo/gaz/subsets/countries/Egypt.owl"
     xmlns:obo="http://purl.obolibrary.org/obo/"
     xmlns:owl="http://www.w3.org/2002/07/owl#"
     xmlns:rdf="http://www.w3.org/1999/02/22-rdf-syntax-ns#"
     xmlns:xml="http://www.w3.org/XML/1998/namespace"
     xmlns:xsd="http://www.w3.org/2001/XMLSchema#"
     xmlns:rdfs="http://www.w3.org/2000/01/rdf-schema#"
     xmlns:oboInOwl="http://www.geneontology.org/formats/oboInOwl#">
    <owl:Ontology rdf:about="http://purl.obolibrary.org/obo/gaz/subsets/countries/Egypt.owl">
        <owl:imports rdf:resource="http://purl.obolibrary.org/obo/gaz/imports/envo_import.owl"/>
        <owl:imports rdf:resource="http://purl.obolibrary.org/obo/gaz/imports/ro_import.owl"/>
    </owl:Ontology>
    


    <!-- 
    ///////////////////////////////////////////////////////////////////////////////////////
    //
    // Annotation properties
    //
    ///////////////////////////////////////////////////////////////////////////////////////
     -->

    


    <!-- http://purl.obolibrary.org/obo/IAO_0000115 -->

    <owl:AnnotationProperty rdf:about="http://purl.obolibrary.org/obo/IAO_0000115"/>
    


    <!-- http://www.geneontology.org/formats/oboInOwl#hasOBONamespace -->

    <owl:AnnotationProperty rdf:about="http://www.geneontology.org/formats/oboInOwl#hasOBONamespace"/>
    


    <!-- http://www.geneontology.org/formats/oboInOwl#id -->

    <owl:AnnotationProperty rdf:about="http://www.geneontology.org/formats/oboInOwl#id"/>
    


    <!-- 
    ///////////////////////////////////////////////////////////////////////////////////////
    //
    // Object Properties
    //
    ///////////////////////////////////////////////////////////////////////////////////////
     -->

    


    <!-- http://purl.obolibrary.org/obo/RO_0001025 -->

    <owl:ObjectProperty rdf:about="http://purl.obolibrary.org/obo/RO_0001025"/>
    


    <!-- 
    ///////////////////////////////////////////////////////////////////////////////////////
    //
    // Classes
    //
    ///////////////////////////////////////////////////////////////////////////////////////
     -->

    


    <!-- http://purl.obolibrary.org/obo/ENVO_00000004 -->

    <owl:Class rdf:about="http://purl.obolibrary.org/obo/ENVO_00000004"/>
    


    <!-- http://purl.obolibrary.org/obo/ENVO_00000032 -->

    <owl:Class rdf:about="http://purl.obolibrary.org/obo/ENVO_00000032"/>
    


    <!-- http://purl.obolibrary.org/obo/ENVO_00000033 -->

    <owl:Class rdf:about="http://purl.obolibrary.org/obo/ENVO_00000033"/>
    


    <!-- http://purl.obolibrary.org/obo/ENVO_00000074 -->

    <owl:Class rdf:about="http://purl.obolibrary.org/obo/ENVO_00000074"/>
    


    <!-- http://purl.obolibrary.org/obo/ENVO_00000220 -->

    <owl:Class rdf:about="http://purl.obolibrary.org/obo/ENVO_00000220"/>
    


    <!-- http://purl.obolibrary.org/obo/ENVO_00000222 -->

    <owl:Class rdf:about="http://purl.obolibrary.org/obo/ENVO_00000222"/>
    


    <!-- http://purl.obolibrary.org/obo/ENVO_00000475 -->

    <owl:Class rdf:about="http://purl.obolibrary.org/obo/ENVO_00000475"/>
    


    <!-- http://purl.obolibrary.org/obo/GAZ_00000645 -->

    <owl:Class rdf:about="http://purl.obolibrary.org/obo/GAZ_00000645">
        <rdfs:subClassOf rdf:resource="http://purl.obolibrary.org/obo/GAZ_00003933"/>
    </owl:Class>
    


    <!-- http://purl.obolibrary.org/obo/GAZ_00000646 -->

    <owl:Class rdf:about="http://purl.obolibrary.org/obo/GAZ_00000646">
        <rdfs:subClassOf rdf:resource="http://purl.obolibrary.org/obo/GAZ_00003933"/>
    </owl:Class>
    


    <!-- http://purl.obolibrary.org/obo/GAZ_00000647 -->

    <owl:Class rdf:about="http://purl.obolibrary.org/obo/GAZ_00000647">
        <rdfs:subClassOf rdf:resource="http://purl.obolibrary.org/obo/GAZ_00003933"/>
    </owl:Class>
    


    <!-- http://purl.obolibrary.org/obo/GAZ_00000648 -->

    <owl:Class rdf:about="http://purl.obolibrary.org/obo/GAZ_00000648">
        <rdfs:subClassOf rdf:resource="http://purl.obolibrary.org/obo/GAZ_00003933"/>
    </owl:Class>
    


    <!-- http://purl.obolibrary.org/obo/GAZ_00000649 -->

    <owl:Class rdf:about="http://purl.obolibrary.org/obo/GAZ_00000649">
        <rdfs:subClassOf rdf:resource="http://purl.obolibrary.org/obo/GAZ_00003933"/>
    </owl:Class>
    


    <!-- http://purl.obolibrary.org/obo/GAZ_00000650 -->

    <owl:Class rdf:about="http://purl.obolibrary.org/obo/GAZ_00000650">
        <rdfs:subClassOf rdf:resource="http://purl.obolibrary.org/obo/GAZ_00003933"/>
    </owl:Class>
    


    <!-- http://purl.obolibrary.org/obo/GAZ_00000651 -->

    <owl:Class rdf:about="http://purl.obolibrary.org/obo/GAZ_00000651">
        <rdfs:subClassOf rdf:resource="http://purl.obolibrary.org/obo/GAZ_00003933"/>
    </owl:Class>
    


    <!-- http://purl.obolibrary.org/obo/GAZ_00000652 -->

    <owl:Class rdf:about="http://purl.obolibrary.org/obo/GAZ_00000652">
        <rdfs:subClassOf rdf:resource="http://purl.obolibrary.org/obo/GAZ_00003933"/>
    </owl:Class>
    


    <!-- http://purl.obolibrary.org/obo/GAZ_00000653 -->

    <owl:Class rdf:about="http://purl.obolibrary.org/obo/GAZ_00000653">
        <rdfs:subClassOf rdf:resource="http://purl.obolibrary.org/obo/GAZ_00003933"/>
    </owl:Class>
    


    <!-- http://purl.obolibrary.org/obo/GAZ_00000654 -->

    <owl:Class rdf:about="http://purl.obolibrary.org/obo/GAZ_00000654">
        <rdfs:subClassOf rdf:resource="http://purl.obolibrary.org/obo/GAZ_00003933"/>
    </owl:Class>
    


    <!-- http://purl.obolibrary.org/obo/GAZ_00000655 -->

    <owl:Class rdf:about="http://purl.obolibrary.org/obo/GAZ_00000655">
        <rdfs:subClassOf rdf:resource="http://purl.obolibrary.org/obo/GAZ_00003933"/>
    </owl:Class>
    


    <!-- http://purl.obolibrary.org/obo/GAZ_00000656 -->

    <owl:Class rdf:about="http://purl.obolibrary.org/obo/GAZ_00000656">
        <rdfs:subClassOf rdf:resource="http://purl.obolibrary.org/obo/GAZ_00003933"/>
    </owl:Class>
    


    <!-- http://purl.obolibrary.org/obo/GAZ_00000657 -->

    <owl:Class rdf:about="http://purl.obolibrary.org/obo/GAZ_00000657">
        <rdfs:subClassOf rdf:resource="http://purl.obolibrary.org/obo/GAZ_00003933"/>
    </owl:Class>
    


    <!-- http://purl.obolibrary.org/obo/GAZ_00000658 -->

    <owl:Class rdf:about="http://purl.obolibrary.org/obo/GAZ_00000658">
        <rdfs:subClassOf rdf:resource="http://purl.obolibrary.org/obo/GAZ_00003933"/>
    </owl:Class>
    


    <!-- http://purl.obolibrary.org/obo/GAZ_00000659 -->

    <owl:Class rdf:about="http://purl.obolibrary.org/obo/GAZ_00000659">
        <rdfs:subClassOf rdf:resource="http://purl.obolibrary.org/obo/GAZ_00003933"/>
    </owl:Class>
    


    <!-- http://purl.obolibrary.org/obo/GAZ_00000660 -->

    <owl:Class rdf:about="http://purl.obolibrary.org/obo/GAZ_00000660">
        <rdfs:subClassOf rdf:resource="http://purl.obolibrary.org/obo/GAZ_00003933"/>
    </owl:Class>
    


    <!-- http://purl.obolibrary.org/obo/GAZ_00000661 -->

    <owl:Class rdf:about="http://purl.obolibrary.org/obo/GAZ_00000661">
        <rdfs:subClassOf rdf:resource="http://purl.obolibrary.org/obo/GAZ_00003933"/>
    </owl:Class>
    


    <!-- http://purl.obolibrary.org/obo/GAZ_00000662 -->

    <owl:Class rdf:about="http://purl.obolibrary.org/obo/GAZ_00000662">
        <rdfs:subClassOf rdf:resource="http://purl.obolibrary.org/obo/GAZ_00003933"/>
    </owl:Class>
    


    <!-- http://purl.obolibrary.org/obo/GAZ_00000663 -->

    <owl:Class rdf:about="http://purl.obolibrary.org/obo/GAZ_00000663">
        <rdfs:subClassOf rdf:resource="http://purl.obolibrary.org/obo/GAZ_00003933"/>
    </owl:Class>
    


    <!-- http://purl.obolibrary.org/obo/GAZ_00000664 -->

    <owl:Class rdf:about="http://purl.obolibrary.org/obo/GAZ_00000664">
        <rdfs:subClassOf rdf:resource="http://purl.obolibrary.org/obo/GAZ_00003933"/>
    </owl:Class>
    


    <!-- http://purl.obolibrary.org/obo/GAZ_00000665 -->

    <owl:Class rdf:about="http://purl.obolibrary.org/obo/GAZ_00000665">
        <rdfs:subClassOf rdf:resource="http://purl.obolibrary.org/obo/GAZ_00003933"/>
    </owl:Class>
    


    <!-- http://purl.obolibrary.org/obo/GAZ_00000666 -->

    <owl:Class rdf:about="http://purl.obolibrary.org/obo/GAZ_00000666">
        <rdfs:subClassOf rdf:resource="http://purl.obolibrary.org/obo/GAZ_00003933"/>
    </owl:Class>
    


    <!-- http://purl.obolibrary.org/obo/GAZ_00000667 -->

    <owl:Class rdf:about="http://purl.obolibrary.org/obo/GAZ_00000667">
        <rdfs:subClassOf rdf:resource="http://purl.obolibrary.org/obo/GAZ_00003933"/>
    </owl:Class>
    


    <!-- http://purl.obolibrary.org/obo/GAZ_00000668 -->

    <owl:Class rdf:about="http://purl.obolibrary.org/obo/GAZ_00000668">
        <rdfs:subClassOf rdf:resource="http://purl.obolibrary.org/obo/GAZ_00003933"/>
    </owl:Class>
    


    <!-- http://purl.obolibrary.org/obo/GAZ_00003933 -->

    <owl:Class rdf:about="http://purl.obolibrary.org/obo/GAZ_00003933"/>
    


    <!-- http://purl.obolibrary.org/obo/GAZ_00003934 -->

    <owl:Class rdf:about="http://purl.obolibrary.org/obo/GAZ_00003934"/>
    


    <!-- http://purl.obolibrary.org/obo/GAZ_00005648 -->

    <owl:Class rdf:about="http://purl.obolibrary.org/obo/GAZ_00005648">
        <rdfs:subClassOf rdf:resource="http://purl.obolibrary.org/obo/GAZ_00005649"/>
    </owl:Class>
    


    <!-- http://purl.obolibrary.org/obo/GAZ_00005649 -->

    <owl:Class rdf:about="http://purl.obolibrary.org/obo/GAZ_00005649"/>
    


    <!-- http://purl.obolibrary.org/obo/GAZ_00012404 -->

    <owl:Class rdf:about="http://purl.obolibrary.org/obo/GAZ_00012404">
        <rdfs:subClassOf rdf:resource="http://purl.obolibrary.org/obo/GAZ_00005649"/>
    </owl:Class>
    


    <!-- http://purl.obolibrary.org/obo/GAZ_00052491 -->

    <owl:Class rdf:about="http://purl.obolibrary.org/obo/GAZ_00052491">
        <rdfs:subClassOf rdf:resource="http://purl.obolibrary.org/obo/GAZ_00005649"/>
    </owl:Class>
    


    <!-- http://purl.obolibrary.org/obo/GAZ_00052492 -->

    <owl:Class rdf:about="http://purl.obolibrary.org/obo/GAZ_00052492">
        <rdfs:subClassOf rdf:resource="http://purl.obolibrary.org/obo/GAZ_00005649"/>
    </owl:Class>
    


    <!-- http://purl.obolibrary.org/obo/GAZ_00052493 -->

    <owl:Class rdf:about="http://purl.obolibrary.org/obo/GAZ_00052493">
        <rdfs:subClassOf rdf:resource="http://purl.obolibrary.org/obo/GAZ_00005649"/>
    </owl:Class>
    


    <!-- http://purl.obolibrary.org/obo/GAZ_00058884 -->

    <owl:Class rdf:about="http://purl.obolibrary.org/obo/GAZ_00058884"/>
    


    <!-- http://purl.obolibrary.org/obo/GAZ_00058885 -->

    <owl:Class rdf:about="http://purl.obolibrary.org/obo/GAZ_00058885">
        <rdfs:subClassOf rdf:resource="http://purl.obolibrary.org/obo/GAZ_00058884"/>
        <obo:IAO_0000115>A cataract on the River Nile in Sudan near the confluence with the Atbara River.</obo:IAO_0000115>
        <oboInOwl:hasOBONamespace>GAZ</oboInOwl:hasOBONamespace>
        <oboInOwl:id>GAZ:00058885</oboInOwl:id>
        <rdfs:label>Fifth Cataract</rdfs:label>
    </owl:Class>
    


    <!-- http://purl.obolibrary.org/obo/GAZ_00058886 -->

    <owl:Class rdf:about="http://purl.obolibrary.org/obo/GAZ_00058886">
        <rdfs:subClassOf rdf:resource="http://purl.obolibrary.org/obo/GAZ_00058884"/>
    </owl:Class>
    


    <!-- http://purl.obolibrary.org/obo/GAZ_00058887 -->

    <owl:Class rdf:about="http://purl.obolibrary.org/obo/GAZ_00058887">
        <rdfs:subClassOf rdf:resource="http://purl.obolibrary.org/obo/GAZ_00058884"/>
        <obo:IAO_0000115>A former cataract on the River Nile in Sudan that was in Nubia and is now submerged in Lake Nasser.</obo:IAO_0000115>
        <oboInOwl:hasOBONamespace>GAZ</oboInOwl:hasOBONamespace>
        <oboInOwl:id>GAZ:00058887</oboInOwl:id>
        <rdfs:label>Second Cataract</rdfs:label>
    </owl:Class>
    


    <!-- http://purl.obolibrary.org/obo/GAZ_00058888 -->

    <owl:Class rdf:about="http://purl.obolibrary.org/obo/GAZ_00058888">
        <rdfs:subClassOf rdf:resource="http://purl.obolibrary.org/obo/GAZ_00058884"/>
        <obo:IAO_0000115>A cataract on the River Nile in Sudan near Tombos.</obo:IAO_0000115>
        <oboInOwl:hasOBONamespace>GAZ</oboInOwl:hasOBONamespace>
        <oboInOwl:id>GAZ:00058888</oboInOwl:id>
        <rdfs:label>Third Cataract</rdfs:label>
    </owl:Class>
    


    <!-- http://purl.obolibrary.org/obo/GAZ_00058889 -->

    <owl:Class rdf:about="http://purl.obolibrary.org/obo/GAZ_00058889">
        <rdfs:subClassOf rdf:resource="http://purl.obolibrary.org/obo/GAZ_00058884"/>
        <obo:IAO_0000115>A cataract on the River Nile in Sudan where it cuts through the Sabaluka pluton near Bagrawiyah.</obo:IAO_0000115>
        <oboInOwl:hasOBONamespace>GAZ</oboInOwl:hasOBONamespace>
        <oboInOwl:id>GAZ:00058889</oboInOwl:id>
        <rdfs:label>Sixth Cataract</rdfs:label>
    </owl:Class>
    


    <!-- http://purl.obolibrary.org/obo/GAZ_00058890 -->

    <owl:Class rdf:about="http://purl.obolibrary.org/obo/GAZ_00058890">
        <rdfs:subClassOf rdf:resource="http://purl.obolibrary.org/obo/GAZ_00058884"/>
    </owl:Class>
    


    <!-- http://purl.obolibrary.org/obo/GAZ_00066400 -->

    <owl:Class rdf:about="http://purl.obolibrary.org/obo/GAZ_00066400">
        <rdfs:subClassOf rdf:resource="http://purl.obolibrary.org/obo/GAZ_00003933"/>
    </owl:Class>
    


    <!-- http://purl.obolibrary.org/obo/GAZ_00089771 -->

    <owl:Class rdf:about="http://purl.obolibrary.org/obo/GAZ_00089771">
        <rdfs:subClassOf rdf:resource="http://purl.obolibrary.org/obo/GAZ_00005649"/>
    </owl:Class>
    


    <!-- http://purl.obolibrary.org/obo/GAZ_00230304 -->

    <owl:Class rdf:about="http://purl.obolibrary.org/obo/GAZ_00230304">
        <rdfs:subClassOf rdf:resource="http://purl.obolibrary.org/obo/GAZ_00003933"/>
    </owl:Class>
    


    <!-- http://purl.obolibrary.org/obo/GAZ_00230305 -->

    <owl:Class rdf:about="http://purl.obolibrary.org/obo/GAZ_00230305">
        <rdfs:subClassOf rdf:resource="http://purl.obolibrary.org/obo/GAZ_00003933"/>
    </owl:Class>
    


    <!-- http://purl.obolibrary.org/obo/GAZ_00230472 -->

    <owl:Class rdf:about="http://purl.obolibrary.org/obo/GAZ_00230472">
        <obo:IAO_0000115>A river. A tributary of the Qechene River.</obo:IAO_0000115>
        <oboInOwl:hasOBONamespace>GAZ</oboInOwl:hasOBONamespace>
        <oboInOwl:id>GAZ:00230472</oboInOwl:id>
        <rdfs:label>Ketama River</rdfs:label>
    </owl:Class>
    


    <!-- http://purl.obolibrary.org/obo/GAZ_00230473 -->

    <owl:Class rdf:about="http://purl.obolibrary.org/obo/GAZ_00230473">
        <obo:IAO_0000115>A river. A tributary of the Qechene River.</obo:IAO_0000115>
        <oboInOwl:hasOBONamespace>GAZ</oboInOwl:hasOBONamespace>
        <oboInOwl:id>GAZ:00230473</oboInOwl:id>
        <rdfs:label>Woia River</rdfs:label>
    </owl:Class>
    


    <!-- 
    ///////////////////////////////////////////////////////////////////////////////////////
    //
    // Individuals
    //
    ///////////////////////////////////////////////////////////////////////////////////////
     -->

    


    <!-- http://purl.obolibrary.org/obo/GAZ_00000561 -->

    <owl:NamedIndividual rdf:about="http://purl.obolibrary.org/obo/GAZ_00000561">
        <obo:RO_0001025 rdf:resource="http://purl.obolibrary.org/obo/GAZ_00003934"/>
        <oboInOwl:hasOBONamespace>GAZ</oboInOwl:hasOBONamespace>
        <oboInOwl:id>GAZ:00000561</oboInOwl:id>
        <rdfs:label>Egypt in Africa</rdfs:label>
    </owl:NamedIndividual>
    


    <!-- http://purl.obolibrary.org/obo/GAZ_00000645 -->

    <owl:NamedIndividual rdf:about="http://purl.obolibrary.org/obo/GAZ_00000645"/>
    


    <!-- http://purl.obolibrary.org/obo/GAZ_00000646 -->

    <owl:NamedIndividual rdf:about="http://purl.obolibrary.org/obo/GAZ_00000646"/>
    


    <!-- http://purl.obolibrary.org/obo/GAZ_00000647 -->

    <owl:NamedIndividual rdf:about="http://purl.obolibrary.org/obo/GAZ_00000647"/>
    


    <!-- http://purl.obolibrary.org/obo/GAZ_00000648 -->

    <owl:NamedIndividual rdf:about="http://purl.obolibrary.org/obo/GAZ_00000648"/>
    


    <!-- http://purl.obolibrary.org/obo/GAZ_00000649 -->

    <owl:NamedIndividual rdf:about="http://purl.obolibrary.org/obo/GAZ_00000649"/>
    


    <!-- http://purl.obolibrary.org/obo/GAZ_00000650 -->

    <owl:NamedIndividual rdf:about="http://purl.obolibrary.org/obo/GAZ_00000650"/>
    


    <!-- http://purl.obolibrary.org/obo/GAZ_00000651 -->

    <owl:NamedIndividual rdf:about="http://purl.obolibrary.org/obo/GAZ_00000651"/>
    


    <!-- http://purl.obolibrary.org/obo/GAZ_00000652 -->

    <owl:NamedIndividual rdf:about="http://purl.obolibrary.org/obo/GAZ_00000652"/>
    


    <!-- http://purl.obolibrary.org/obo/GAZ_00000653 -->

    <owl:NamedIndividual rdf:about="http://purl.obolibrary.org/obo/GAZ_00000653"/>
    


    <!-- http://purl.obolibrary.org/obo/GAZ_00000654 -->

    <owl:NamedIndividual rdf:about="http://purl.obolibrary.org/obo/GAZ_00000654"/>
    


    <!-- http://purl.obolibrary.org/obo/GAZ_00000655 -->

    <owl:NamedIndividual rdf:about="http://purl.obolibrary.org/obo/GAZ_00000655"/>
    


    <!-- http://purl.obolibrary.org/obo/GAZ_00000656 -->

    <owl:NamedIndividual rdf:about="http://purl.obolibrary.org/obo/GAZ_00000656"/>
    


    <!-- http://purl.obolibrary.org/obo/GAZ_00000657 -->

    <owl:NamedIndividual rdf:about="http://purl.obolibrary.org/obo/GAZ_00000657"/>
    


    <!-- http://purl.obolibrary.org/obo/GAZ_00000658 -->

    <owl:NamedIndividual rdf:about="http://purl.obolibrary.org/obo/GAZ_00000658"/>
    


    <!-- http://purl.obolibrary.org/obo/GAZ_00000659 -->

    <owl:NamedIndividual rdf:about="http://purl.obolibrary.org/obo/GAZ_00000659"/>
    


    <!-- http://purl.obolibrary.org/obo/GAZ_00000660 -->

    <owl:NamedIndividual rdf:about="http://purl.obolibrary.org/obo/GAZ_00000660"/>
    


    <!-- http://purl.obolibrary.org/obo/GAZ_00000661 -->

    <owl:NamedIndividual rdf:about="http://purl.obolibrary.org/obo/GAZ_00000661"/>
    


    <!-- http://purl.obolibrary.org/obo/GAZ_00000662 -->

    <owl:NamedIndividual rdf:about="http://purl.obolibrary.org/obo/GAZ_00000662"/>
    


    <!-- http://purl.obolibrary.org/obo/GAZ_00000663 -->

    <owl:NamedIndividual rdf:about="http://purl.obolibrary.org/obo/GAZ_00000663"/>
    


    <!-- http://purl.obolibrary.org/obo/GAZ_00000664 -->

    <owl:NamedIndividual rdf:about="http://purl.obolibrary.org/obo/GAZ_00000664"/>
    


    <!-- http://purl.obolibrary.org/obo/GAZ_00000665 -->

    <owl:NamedIndividual rdf:about="http://purl.obolibrary.org/obo/GAZ_00000665"/>
    


    <!-- http://purl.obolibrary.org/obo/GAZ_00000666 -->

    <owl:NamedIndividual rdf:about="http://purl.obolibrary.org/obo/GAZ_00000666"/>
    


    <!-- http://purl.obolibrary.org/obo/GAZ_00000667 -->

    <owl:NamedIndividual rdf:about="http://purl.obolibrary.org/obo/GAZ_00000667"/>
    


    <!-- http://purl.obolibrary.org/obo/GAZ_00000668 -->

    <owl:NamedIndividual rdf:about="http://purl.obolibrary.org/obo/GAZ_00000668"/>
    


    <!-- http://purl.obolibrary.org/obo/GAZ_00000669 -->

    <owl:NamedIndividual rdf:about="http://purl.obolibrary.org/obo/GAZ_00000669">
        <obo:IAO_0000115>One of the governorates of Egypt. It is in the east of the country, covering the northern half of the Sinai Peninsula. Its capital is Arish.</obo:IAO_0000115>
        <oboInOwl:hasOBONamespace>GAZ</oboInOwl:hasOBONamespace>
        <oboInOwl:id>GAZ:00000669</oboInOwl:id>
        <rdfs:label>North Sinai Governorate</rdfs:label>
    </owl:NamedIndividual>
    


    <!-- http://purl.obolibrary.org/obo/GAZ_00000670 -->

    <owl:NamedIndividual rdf:about="http://purl.obolibrary.org/obo/GAZ_00000670">
        <obo:IAO_0000115>One of the governorates of Egypt. It is in the east of the country, covering the southern half of the Sinai Peninsula.</obo:IAO_0000115>
        <oboInOwl:hasOBONamespace>GAZ</oboInOwl:hasOBONamespace>
        <oboInOwl:id>GAZ:00000670</oboInOwl:id>
        <rdfs:label>South Sinai Governorate</rdfs:label>
    </owl:NamedIndividual>
    


    <!-- http://purl.obolibrary.org/obo/GAZ_00000855 -->

    <owl:NamedIndividual rdf:about="http://purl.obolibrary.org/obo/GAZ_00000855">
        <obo:RO_0001025 rdf:resource="http://purl.obolibrary.org/obo/GAZ_00003934"/>
        <oboInOwl:hasOBONamespace>GAZ</oboInOwl:hasOBONamespace>
        <oboInOwl:id>GAZ:00000855</oboInOwl:id>
        <rdfs:label>Egypt in Asia</rdfs:label>
    </owl:NamedIndividual>
    


    <!-- http://purl.obolibrary.org/obo/GAZ_00002456 -->

    <owl:NamedIndividual rdf:about="http://purl.obolibrary.org/obo/GAZ_00002456">
        <obo:IAO_0000115>A sea situated between the coasts of Africa and the Arabian Peninsula, are the following: On the North: A line joining the coast of Africa, in Egypt, eastward, along the parallel of 27 Degrees 27 Minutes N, to the southern extremity of Shaker Island (27 Degrees 27 Minutes N - 34 Degrees 02 Minutes 10 Seconds E), and northeastward to Cape Muhammad (27 Degrees 43 Minutes 35 Seconds N - 34 Degrees 15 Minutes E), the southern extremity of the Sinai Peninsula (the common limit with the Gulf of Suez); thence from Cape Muhammad northeastward, along the southern coast of the Sinai Peninsula, to the parallel of 27 Degrees 54 Minutes 50 Seconds N; thence a line joining the southern coast of the Sinai Peninsula eastward, along the parallel of 27 Degrees 54 Minutes 50 Seconds N, to the southwestern extremity of T Degrees r Degrees n Island (27 Degrees 54 Minutes 50 Seconds N - 34 Degrees 33 Minutes E); thence from the southwestern extremity of T Degrees r Degrees n Island northward, through this island, to position 27 Degrees 58 Minutes 10 Seconds N - 34 Degrees 35 Minutes E), on the northeastern coast thereof; and thence a line joining this position northeastward to Cape Al Qa Degrees bah (28 Degrees 01 Minutes 30 Seconds N - 34 Degrees 37 Minutes 15 Seconds E), in Saudi Arabia (the common limit with the Gulf of Aqaba). On the East: From Cape Al Qa Degrees bah, in Saudi Arabia, southeastward, along the coast of the Arabian Peninsula, to Hisn Mur Degrees d (12 Degrees 40 Minutes 20 Seconds N - 43 Degrees 30 Minutes 20 Seconds E), in Southern Yemen. On the South: A line joining Hisn Mur Degrees d, in Southern Yemen, southwestward to Cape Si Ane (12 Degrees 28 Minutes 50 Seconds N - 43 Degrees 19 Minutes 10 Seconds E), in Djibouti (the common limit with the Gulf of Aden). On the West: From Cape Si Ane, in Djibouti, northwestward, along the coast of Africa, to the parallel of 27 Degrees 27 Minutes N, in Egypt.</obo:IAO_0000115>
        <oboInOwl:hasOBONamespace>GAZ</oboInOwl:hasOBONamespace>
        <oboInOwl:id>GAZ:00002456</oboInOwl:id>
        <rdfs:label>Red Sea</rdfs:label>
    </owl:NamedIndividual>
    


    <!-- http://purl.obolibrary.org/obo/GAZ_00003933 -->

    <owl:NamedIndividual rdf:about="http://purl.obolibrary.org/obo/GAZ_00003933">
        <obo:RO_0001025 rdf:resource="http://purl.obolibrary.org/obo/GAZ_00000561"/>
    </owl:NamedIndividual>
    


    <!-- http://purl.obolibrary.org/obo/GAZ_00003934 -->

    <owl:NamedIndividual rdf:about="http://purl.obolibrary.org/obo/GAZ_00003934"/>
    


    <!-- http://purl.obolibrary.org/obo/GAZ_00004033 -->

    <owl:NamedIndividual rdf:about="http://purl.obolibrary.org/obo/GAZ_00004033">
        <oboInOwl:hasOBONamespace>GAZ</oboInOwl:hasOBONamespace>
        <oboInOwl:id>GAZ:00004033</oboInOwl:id>
        <rdfs:label>Northern Sahara Desert</rdfs:label>
    </owl:NamedIndividual>
    


    <!-- http://purl.obolibrary.org/obo/GAZ_00004037 -->

    <owl:NamedIndividual rdf:about="http://purl.obolibrary.org/obo/GAZ_00004037">
        <obo:RO_0001025 rdf:resource="http://purl.obolibrary.org/obo/GAZ_00000662"/>
        <obo:RO_0001025 rdf:resource="http://purl.obolibrary.org/obo/GAZ_00144637"/>
        <obo:IAO_0000115>A small shore island in the Red Sea. It is owned by Egypt and can be found at the northern entrance to Foul Bay.</obo:IAO_0000115>
        <oboInOwl:hasOBONamespace>GAZ</oboInOwl:hasOBONamespace>
        <oboInOwl:id>GAZ:00004037</oboInOwl:id>
        <rdfs:label>Mukawwar Island</rdfs:label>
    </owl:NamedIndividual>
    


    <!-- http://purl.obolibrary.org/obo/GAZ_00005648 -->

    <owl:NamedIndividual rdf:about="http://purl.obolibrary.org/obo/GAZ_00005648">
        <obo:RO_0001025 rdf:resource="http://purl.obolibrary.org/obo/GAZ_00000663"/>
    </owl:NamedIndividual>
    


    <!-- http://purl.obolibrary.org/obo/GAZ_00005649 -->

    <owl:NamedIndividual rdf:about="http://purl.obolibrary.org/obo/GAZ_00005649">
        <obo:RO_0001025 rdf:resource="http://purl.obolibrary.org/obo/GAZ_00003934"/>
    </owl:NamedIndividual>
    


    <!-- http://purl.obolibrary.org/obo/GAZ_00005650 -->

    <owl:NamedIndividual rdf:about="http://purl.obolibrary.org/obo/GAZ_00005650">
        <obo:RO_0001025 rdf:resource="http://purl.obolibrary.org/obo/GAZ_00000650"/>
        <obo:IAO_0000115>The site of Amarna is located on the east bank of the Nile River in the modern Egyptian province of Minya, some 58 km south of the city of al-Minya, 312 km south of the Egyptian capital Cairo and 402 km north of Luxor. The site of Amarna includes several modern villages, chief of which are el-Till in the north and el-Hagg Qandil in the south.</obo:IAO_0000115>
        <oboInOwl:hasOBONamespace>GAZ</oboInOwl:hasOBONamespace>
        <oboInOwl:id>GAZ:00005650</oboInOwl:id>
        <rdfs:label>Amarna</rdfs:label>
    </owl:NamedIndividual>
    


    <!-- http://purl.obolibrary.org/obo/GAZ_00005876 -->

    <owl:NamedIndividual rdf:about="http://purl.obolibrary.org/obo/GAZ_00005876">
        <rdf:type rdf:resource="http://purl.obolibrary.org/obo/ENVO_00000220"/>
        <obo:RO_0001025 rdf:resource="http://purl.obolibrary.org/obo/GAZ_00053597"/>
        <obo:IAO_0000115>An island group in the Red Sea. Most of them are a part of Yemen, but before 1998-1999 they were claimed by Eritrea as well. They are formed from a series of volcanic vents along a NE-SW trend, and include the Holocene Great Hanish, Little Hanish, and many other small islands and submarine shoals.</obo:IAO_0000115>
        <oboInOwl:hasOBONamespace>GAZ</oboInOwl:hasOBONamespace>
        <oboInOwl:id>GAZ:00005876</oboInOwl:id>
        <rdfs:label>Hanish Islands</rdfs:label>
    </owl:NamedIndividual>
    


    <!-- http://purl.obolibrary.org/obo/GAZ_00005877 -->

    <owl:NamedIndividual rdf:about="http://purl.obolibrary.org/obo/GAZ_00005877">
        <obo:RO_0001025 rdf:resource="http://purl.obolibrary.org/obo/GAZ_00002456"/>
        <obo:IAO_0000115>A &quot;shelf island&quot; located in the shallow waters of the Arabian peninsula&apos;s continental shelf with coral reefs surrounding three sides of the island.</obo:IAO_0000115>
        <oboInOwl:hasOBONamespace>GAZ</oboInOwl:hasOBONamespace>
        <oboInOwl:id>GAZ:00005877</oboInOwl:id>
        <rdfs:label>Kamaran Island</rdfs:label>
    </owl:NamedIndividual>
    


    <!-- http://purl.obolibrary.org/obo/GAZ_00005878 -->

    <owl:NamedIndividual rdf:about="http://purl.obolibrary.org/obo/GAZ_00005878">
        <rdf:type rdf:resource="http://purl.obolibrary.org/obo/ENVO_00000222"/>
        <obo:RO_0001025 rdf:resource="http://purl.obolibrary.org/obo/GAZ_00051269"/>
        <obo:IAO_0000115>A volcanic island located in the Strait of Mandeb at the southern entrance into the Red Sea off the southwestern coast of Yemen.</obo:IAO_0000115>
        <oboInOwl:hasOBONamespace>GAZ</oboInOwl:hasOBONamespace>
        <oboInOwl:id>GAZ:00005878</oboInOwl:id>
        <rdfs:label>Perim</rdfs:label>
    </owl:NamedIndividual>
    


    <!-- http://purl.obolibrary.org/obo/GAZ_00005879 -->

    <owl:NamedIndividual rdf:about="http://purl.obolibrary.org/obo/GAZ_00005879">
        <obo:RO_0001025 rdf:resource="http://purl.obolibrary.org/obo/GAZ_00053597"/>
        <obo:IAO_0000115>An island of Yemen in the Red Sea. It lies the coasts of Yemen and Eritrea near the Bab-el-Mandeb straits, which connect the Red Sea to the Gulf of Aden. Despite its proximity to the African continent, it is considered an island of Asia because it sits on the Asian continental shelf. A shield volcano.</obo:IAO_0000115>
        <oboInOwl:hasOBONamespace>GAZ</oboInOwl:hasOBONamespace>
        <oboInOwl:id>GAZ:00005879</oboInOwl:id>
        <rdfs:label>Zuqar Island</rdfs:label>
    </owl:NamedIndividual>
    


    <!-- http://purl.obolibrary.org/obo/GAZ_00007521 -->

    <owl:NamedIndividual rdf:about="http://purl.obolibrary.org/obo/GAZ_00007521">
        <obo:RO_0001025 rdf:resource="http://purl.obolibrary.org/obo/GAZ_00000655"/>
        <obo:IAO_0000115>An administrative region (markuz) of Beheira Governorate. A region that has a series of evaporitic lakes that lie to the west of Cairo, close to the Cairo-Alexandria road. The lakes, while containing significant water in the winter months, dry out almost completely in the summer forming thick deposits of sodium salts, mostly chlorides, sulphides and carbonates.</obo:IAO_0000115>
        <oboInOwl:hasOBONamespace>GAZ</oboInOwl:hasOBONamespace>
        <oboInOwl:id>GAZ:00007521</oboInOwl:id>
        <rdfs:label>Wadi El Natrun Region</rdfs:label>
    </owl:NamedIndividual>
    


    <!-- http://purl.obolibrary.org/obo/GAZ_00007522 -->

    <owl:NamedIndividual rdf:about="http://purl.obolibrary.org/obo/GAZ_00007522">
        <obo:RO_0001025 rdf:resource="http://purl.obolibrary.org/obo/GAZ_00230319"/>
        <obo:IAO_0000115>A hypersaline lake.</obo:IAO_0000115>
        <oboInOwl:hasOBONamespace>GAZ</oboInOwl:hasOBONamespace>
        <oboInOwl:id>GAZ:00007522</oboInOwl:id>
        <rdfs:label>Abu-Gabara Lake</rdfs:label>
    </owl:NamedIndividual>
    


    <!-- http://purl.obolibrary.org/obo/GAZ_00007862 -->

    <owl:NamedIndividual rdf:about="http://purl.obolibrary.org/obo/GAZ_00007862">
        <rdf:type rdf:resource="http://purl.obolibrary.org/obo/ENVO_00000032"/>
        <obo:IAO_0000115>A gulf situated northeastward and adjacent to the Red Sea, bounded by the coasts of Sinai Peninsula and Arabian Peninsula. Its southern limit with the Red Sea (in the Strait of T Degrees r Degrees n) is the following: A line joining Cape Al Qa Degrees bah (28 Degrees 01430 Seconds N - 34 Degrees 37 Minutes 15 Seconds E), in Saudi Arabia, southwestward to position 27 Degrees 58 Minutes 10 Seconds N - 34 Degrees 35 Minutes E) on the coast of T Degrees r Degrees n Island; thence from this position southward, through T Degrees r Degrees n Island, to its southwestern extremity (27 Degrees 54 Minutes 50 Seconds N - 34 Degrees 33 Minutes E); and thence from the southwestern extremity of T Degrees r Degrees n Island westward, along the parallel of 27 Degrees 54 Minutes 50 Seconds N, to the coast of Sinai Peninsula, in Egypt.</obo:IAO_0000115>
        <oboInOwl:hasOBONamespace>GAZ</oboInOwl:hasOBONamespace>
        <oboInOwl:id>GAZ:00007862</oboInOwl:id>
        <rdfs:label>Gulf of Aqaba</rdfs:label>
    </owl:NamedIndividual>
    


    <!-- http://purl.obolibrary.org/obo/GAZ_00008153 -->

    <owl:NamedIndividual rdf:about="http://purl.obolibrary.org/obo/GAZ_00008153">
        <rdf:type rdf:resource="http://purl.obolibrary.org/obo/ENVO_00000033"/>
        <obo:RO_0001025 rdf:resource="http://purl.obolibrary.org/obo/GAZ_00002456"/>
        <obo:IAO_0000115>A submarine basin. A pool of hot saline brine at the bottom of the central rift in the Red Sea.</obo:IAO_0000115>
        <oboInOwl:hasOBONamespace>GAZ</oboInOwl:hasOBONamespace>
        <oboInOwl:id>GAZ:00008153</oboInOwl:id>
        <rdfs:label>Atlantis II Deep</rdfs:label>
    </owl:NamedIndividual>
    


    <!-- http://purl.obolibrary.org/obo/GAZ_00008590 -->

    <owl:NamedIndividual rdf:about="http://purl.obolibrary.org/obo/GAZ_00008590">
        <obo:RO_0001025 rdf:resource="http://purl.obolibrary.org/obo/GAZ_00230319"/>
        <obo:IAO_0000115>A hypersaline lake.</obo:IAO_0000115>
        <oboInOwl:hasOBONamespace>GAZ</oboInOwl:hasOBONamespace>
        <oboInOwl:id>GAZ:00008590</oboInOwl:id>
        <rdfs:label>Bosa Lake</rdfs:label>
    </owl:NamedIndividual>
    


    <!-- http://purl.obolibrary.org/obo/GAZ_00008592 -->

    <owl:NamedIndividual rdf:about="http://purl.obolibrary.org/obo/GAZ_00008592">
        <obo:RO_0001025 rdf:resource="http://purl.obolibrary.org/obo/GAZ_00000661"/>
        <oboInOwl:hasOBONamespace>GAZ</oboInOwl:hasOBONamespace>
        <oboInOwl:id>GAZ:00008592</oboInOwl:id>
        <rdfs:label>Kafr-Hamsa</rdfs:label>
    </owl:NamedIndividual>
    


    <!-- http://purl.obolibrary.org/obo/GAZ_00009408 -->

    <owl:NamedIndividual rdf:about="http://purl.obolibrary.org/obo/GAZ_00009408">
        <obo:RO_0001025 rdf:resource="http://purl.obolibrary.org/obo/GAZ_00002456"/>
        <oboInOwl:hasOBONamespace>GAZ</oboInOwl:hasOBONamespace>
        <oboInOwl:id>GAZ:00009408</oboInOwl:id>
        <rdfs:label>Suakin Archipelago</rdfs:label>
    </owl:NamedIndividual>
    


    <!-- http://purl.obolibrary.org/obo/GAZ_00009683 -->

    <owl:NamedIndividual rdf:about="http://purl.obolibrary.org/obo/GAZ_00009683">
        <rdf:type rdf:resource="http://purl.obolibrary.org/obo/ENVO_00000220"/>
        <obo:RO_0001025 rdf:resource="http://purl.obolibrary.org/obo/GAZ_00002456"/>
        <obo:IAO_0000115>An island group located in the Red Sea near Massawa, Eritrea. It consists of two large and 124 small islands.</obo:IAO_0000115>
        <oboInOwl:hasOBONamespace>GAZ</oboInOwl:hasOBONamespace>
        <oboInOwl:id>GAZ:00009683</oboInOwl:id>
        <rdfs:label>Dahlak Archipelago</rdfs:label>
    </owl:NamedIndividual>
    


    <!-- http://purl.obolibrary.org/obo/GAZ_00009949 -->

    <owl:NamedIndividual rdf:about="http://purl.obolibrary.org/obo/GAZ_00009949">
        <obo:IAO_0000115>The delta formed in Northern Egypt where the Nile River spreads out and drains into the Mediterranean Sea. It is one of the world&apos;s largest river delta, from Alexandria in the west to Port Said in the east, it covers some 240 km of Mediterranean coastline.</obo:IAO_0000115>
        <oboInOwl:hasOBONamespace>GAZ</oboInOwl:hasOBONamespace>
        <oboInOwl:id>GAZ:00009949</oboInOwl:id>
        <rdfs:label>Nile Delta</rdfs:label>
    </owl:NamedIndividual>
    


    <!-- http://purl.obolibrary.org/obo/GAZ_00011760 -->

    <owl:NamedIndividual rdf:about="http://purl.obolibrary.org/obo/GAZ_00011760">
        <obo:RO_0001025 rdf:resource="http://purl.obolibrary.org/obo/GAZ_00230319"/>
        <obo:IAO_0000115>A saline lake.</obo:IAO_0000115>
        <oboInOwl:hasOBONamespace>GAZ</oboInOwl:hasOBONamespace>
        <oboInOwl:id>GAZ:00011760</oboInOwl:id>
        <rdfs:label>Lake Hamra</rdfs:label>
    </owl:NamedIndividual>
    


    <!-- http://purl.obolibrary.org/obo/GAZ_00011777 -->

    <owl:NamedIndividual rdf:about="http://purl.obolibrary.org/obo/GAZ_00011777">
        <obo:RO_0001025 rdf:resource="http://purl.obolibrary.org/obo/GAZ_00230319"/>
        <obo:IAO_0000115>A saline lake.</obo:IAO_0000115>
        <oboInOwl:hasOBONamespace>GAZ</oboInOwl:hasOBONamespace>
        <oboInOwl:id>GAZ:00011777</oboInOwl:id>
        <rdfs:label>Birket Umm Risha</rdfs:label>
    </owl:NamedIndividual>
    


    <!-- http://purl.obolibrary.org/obo/GAZ_00011778 -->

    <owl:NamedIndividual rdf:about="http://purl.obolibrary.org/obo/GAZ_00011778">
        <obo:RO_0001025 rdf:resource="http://purl.obolibrary.org/obo/GAZ_00230319"/>
        <obo:IAO_0000115>A saline lake.</obo:IAO_0000115>
        <oboInOwl:hasOBONamespace>GAZ</oboInOwl:hasOBONamespace>
        <oboInOwl:id>GAZ:00011778</oboInOwl:id>
        <rdfs:label>Birket el Gaar</rdfs:label>
    </owl:NamedIndividual>
    


    <!-- http://purl.obolibrary.org/obo/GAZ_00011779 -->

    <owl:NamedIndividual rdf:about="http://purl.obolibrary.org/obo/GAZ_00011779">
        <obo:RO_0001025 rdf:resource="http://purl.obolibrary.org/obo/GAZ_00230319"/>
        <oboInOwl:hasOBONamespace>GAZ</oboInOwl:hasOBONamespace>
        <oboInOwl:id>GAZ:00011779</oboInOwl:id>
        <rdfs:label>Al Buhayrah</rdfs:label>
    </owl:NamedIndividual>
    


    <!-- http://purl.obolibrary.org/obo/GAZ_00011780 -->

    <owl:NamedIndividual rdf:about="http://purl.obolibrary.org/obo/GAZ_00011780">
        <obo:RO_0001025 rdf:resource="http://purl.obolibrary.org/obo/GAZ_00230319"/>
        <obo:IAO_0000115>A saline lake.</obo:IAO_0000115>
        <oboInOwl:hasOBONamespace>GAZ</oboInOwl:hasOBONamespace>
        <oboInOwl:id>GAZ:00011780</oboInOwl:id>
        <rdfs:label>Birket el Beida</rdfs:label>
    </owl:NamedIndividual>
    


    <!-- http://purl.obolibrary.org/obo/GAZ_00011781 -->

    <owl:NamedIndividual rdf:about="http://purl.obolibrary.org/obo/GAZ_00011781">
        <obo:RO_0001025 rdf:resource="http://purl.obolibrary.org/obo/GAZ_00230319"/>
        <oboInOwl:hasOBONamespace>GAZ</oboInOwl:hasOBONamespace>
        <oboInOwl:id>GAZ:00011781</oboInOwl:id>
        <rdfs:label>Birket el Zugm</rdfs:label>
    </owl:NamedIndividual>
    


    <!-- http://purl.obolibrary.org/obo/GAZ_00011804 -->

    <owl:NamedIndividual rdf:about="http://purl.obolibrary.org/obo/GAZ_00011804">
        <obo:RO_0001025 rdf:resource="http://purl.obolibrary.org/obo/GAZ_00230319"/>
        <oboInOwl:hasOBONamespace>GAZ</oboInOwl:hasOBONamespace>
        <oboInOwl:id>GAZ:00011804</oboInOwl:id>
        <rdfs:label>Lake Fazda</rdfs:label>
    </owl:NamedIndividual>
    


    <!-- http://purl.obolibrary.org/obo/GAZ_00012404 -->

    <owl:NamedIndividual rdf:about="http://purl.obolibrary.org/obo/GAZ_00012404">
        <obo:RO_0001025 rdf:resource="http://purl.obolibrary.org/obo/GAZ_00066397"/>
    </owl:NamedIndividual>
    


    <!-- http://purl.obolibrary.org/obo/GAZ_00030898 -->

    <owl:NamedIndividual rdf:about="http://purl.obolibrary.org/obo/GAZ_00030898">
        <obo:RO_0001025 rdf:resource="http://purl.obolibrary.org/obo/GAZ_00000656"/>
        <obo:IAO_0000115>An administrative region (markaz) of Dakahlia Governorate.</obo:IAO_0000115>
        <oboInOwl:hasOBONamespace>GAZ</oboInOwl:hasOBONamespace>
        <oboInOwl:id>GAZ:00030898</oboInOwl:id>
        <rdfs:label>Bani &apos;Ebeid Region</rdfs:label>
    </owl:NamedIndividual>
    


    <!-- http://purl.obolibrary.org/obo/GAZ_00030899 -->

    <owl:NamedIndividual rdf:about="http://purl.obolibrary.org/obo/GAZ_00030899">
        <obo:RO_0001025 rdf:resource="http://purl.obolibrary.org/obo/GAZ_00000656"/>
        <obo:IAO_0000115>An administrative region (markaz) of Dakahlia Governorate.</obo:IAO_0000115>
        <oboInOwl:hasOBONamespace>GAZ</oboInOwl:hasOBONamespace>
        <oboInOwl:id>GAZ:00030899</oboInOwl:id>
        <rdfs:label>Temayy Al Amdeed Region</rdfs:label>
    </owl:NamedIndividual>
    


    <!-- http://purl.obolibrary.org/obo/GAZ_00030900 -->

    <owl:NamedIndividual rdf:about="http://purl.obolibrary.org/obo/GAZ_00030900">
        <obo:RO_0001025 rdf:resource="http://purl.obolibrary.org/obo/GAZ_00000656"/>
        <obo:IAO_0000115>An administrative region (markaz) of Dakahlia Governorate.</obo:IAO_0000115>
        <oboInOwl:hasOBONamespace>GAZ</oboInOwl:hasOBONamespace>
        <oboInOwl:id>GAZ:00030900</oboInOwl:id>
        <rdfs:label>Al Gammaliyyah Region</rdfs:label>
    </owl:NamedIndividual>
    


    <!-- http://purl.obolibrary.org/obo/GAZ_00030901 -->

    <owl:NamedIndividual rdf:about="http://purl.obolibrary.org/obo/GAZ_00030901">
        <obo:RO_0001025 rdf:resource="http://purl.obolibrary.org/obo/GAZ_00000656"/>
        <obo:IAO_0000115>An administrative region (markaz) of Dakahlia Governorate.</obo:IAO_0000115>
        <oboInOwl:hasOBONamespace>GAZ</oboInOwl:hasOBONamespace>
        <oboInOwl:id>GAZ:00030901</oboInOwl:id>
        <rdfs:label>Al Mansoura Region</rdfs:label>
    </owl:NamedIndividual>
    


    <!-- http://purl.obolibrary.org/obo/GAZ_00030902 -->

    <owl:NamedIndividual rdf:about="http://purl.obolibrary.org/obo/GAZ_00030902">
        <obo:RO_0001025 rdf:resource="http://purl.obolibrary.org/obo/GAZ_00000656"/>
        <obo:IAO_0000115>An administrative region (markaz) of Dakahlia Governorate.</obo:IAO_0000115>
        <oboInOwl:hasOBONamespace>GAZ</oboInOwl:hasOBONamespace>
        <oboInOwl:id>GAZ:00030902</oboInOwl:id>
        <rdfs:label>Al Matariyyah Region</rdfs:label>
    </owl:NamedIndividual>
    


    <!-- http://purl.obolibrary.org/obo/GAZ_00030903 -->

    <owl:NamedIndividual rdf:about="http://purl.obolibrary.org/obo/GAZ_00030903">
        <obo:RO_0001025 rdf:resource="http://purl.obolibrary.org/obo/GAZ_00000656"/>
        <obo:IAO_0000115>An administrative region (markaz) of Dakahlia Governorate.</obo:IAO_0000115>
        <oboInOwl:hasOBONamespace>GAZ</oboInOwl:hasOBONamespace>
        <oboInOwl:id>GAZ:00030903</oboInOwl:id>
        <rdfs:label>Al Manzalah Region</rdfs:label>
    </owl:NamedIndividual>
    


    <!-- http://purl.obolibrary.org/obo/GAZ_00030904 -->

    <owl:NamedIndividual rdf:about="http://purl.obolibrary.org/obo/GAZ_00030904">
        <obo:RO_0001025 rdf:resource="http://purl.obolibrary.org/obo/GAZ_00000656"/>
        <obo:IAO_0000115>An administrative region (markaz) of Dakahlia Governorate.</obo:IAO_0000115>
        <oboInOwl:hasOBONamespace>GAZ</oboInOwl:hasOBONamespace>
        <oboInOwl:id>GAZ:00030904</oboInOwl:id>
        <rdfs:label>Meit Salseel Region</rdfs:label>
    </owl:NamedIndividual>
    


    <!-- http://purl.obolibrary.org/obo/GAZ_00030905 -->

    <owl:NamedIndividual rdf:about="http://purl.obolibrary.org/obo/GAZ_00030905">
        <obo:RO_0001025 rdf:resource="http://purl.obolibrary.org/obo/GAZ_00000656"/>
        <obo:IAO_0000115>An administrative region (markaz) of Dakahlia Governorate.</obo:IAO_0000115>
        <oboInOwl:hasOBONamespace>GAZ</oboInOwl:hasOBONamespace>
        <oboInOwl:id>GAZ:00030905</oboInOwl:id>
        <rdfs:label>Aga Region</rdfs:label>
    </owl:NamedIndividual>
    


    <!-- http://purl.obolibrary.org/obo/GAZ_00030906 -->

    <owl:NamedIndividual rdf:about="http://purl.obolibrary.org/obo/GAZ_00030906">
        <obo:RO_0001025 rdf:resource="http://purl.obolibrary.org/obo/GAZ_00000656"/>
        <obo:IAO_0000115>An administrative region (markaz) of Dakahlia Governorate.</obo:IAO_0000115>
        <oboInOwl:hasOBONamespace>GAZ</oboInOwl:hasOBONamespace>
        <oboInOwl:id>GAZ:00030906</oboInOwl:id>
        <rdfs:label>Dikirnis Region</rdfs:label>
    </owl:NamedIndividual>
    


    <!-- http://purl.obolibrary.org/obo/GAZ_00030907 -->

    <owl:NamedIndividual rdf:about="http://purl.obolibrary.org/obo/GAZ_00030907">
        <obo:RO_0001025 rdf:resource="http://purl.obolibrary.org/obo/GAZ_00000656"/>
        <obo:IAO_0000115>An administrative region (markaz) of Dakahlia Governorate.</obo:IAO_0000115>
        <oboInOwl:hasOBONamespace>GAZ</oboInOwl:hasOBONamespace>
        <oboInOwl:id>GAZ:00030907</oboInOwl:id>
        <rdfs:label>Menyat Al Nasr Region</rdfs:label>
    </owl:NamedIndividual>
    


    <!-- http://purl.obolibrary.org/obo/GAZ_00030908 -->

    <owl:NamedIndividual rdf:about="http://purl.obolibrary.org/obo/GAZ_00030908">
        <obo:RO_0001025 rdf:resource="http://purl.obolibrary.org/obo/GAZ_00000656"/>
        <obo:IAO_0000115>An administrative region (markaz) of Dakahlia Governorate.</obo:IAO_0000115>
        <oboInOwl:hasOBONamespace>GAZ</oboInOwl:hasOBONamespace>
        <oboInOwl:id>GAZ:00030908</oboInOwl:id>
        <rdfs:label>Mahallat Damanah Region</rdfs:label>
    </owl:NamedIndividual>
    


    <!-- http://purl.obolibrary.org/obo/GAZ_00030909 -->

    <owl:NamedIndividual rdf:about="http://purl.obolibrary.org/obo/GAZ_00030909">
        <obo:RO_0001025 rdf:resource="http://purl.obolibrary.org/obo/GAZ_00000656"/>
        <obo:IAO_0000115>An administrative region (markaz) of Dakahlia Governorate.</obo:IAO_0000115>
        <oboInOwl:hasOBONamespace>GAZ</oboInOwl:hasOBONamespace>
        <oboInOwl:id>GAZ:00030909</oboInOwl:id>
        <rdfs:label>Belqas Region</rdfs:label>
    </owl:NamedIndividual>
    


    <!-- http://purl.obolibrary.org/obo/GAZ_00030910 -->

    <owl:NamedIndividual rdf:about="http://purl.obolibrary.org/obo/GAZ_00030910">
        <obo:RO_0001025 rdf:resource="http://purl.obolibrary.org/obo/GAZ_00000656"/>
        <obo:IAO_0000115>An administrative region (markaz) of Dakahlia Governorate.</obo:IAO_0000115>
        <oboInOwl:hasOBONamespace>GAZ</oboInOwl:hasOBONamespace>
        <oboInOwl:id>GAZ:00030910</oboInOwl:id>
        <rdfs:label>Al Senbellawein Region</rdfs:label>
    </owl:NamedIndividual>
    


    <!-- http://purl.obolibrary.org/obo/GAZ_00030911 -->

    <owl:NamedIndividual rdf:about="http://purl.obolibrary.org/obo/GAZ_00030911">
        <obo:RO_0001025 rdf:resource="http://purl.obolibrary.org/obo/GAZ_00000656"/>
        <obo:IAO_0000115>An administrative region (markaz) of Dakahlia Governorate.</obo:IAO_0000115>
        <oboInOwl:hasOBONamespace>GAZ</oboInOwl:hasOBONamespace>
        <oboInOwl:id>GAZ:00030911</oboInOwl:id>
        <rdfs:label>Sherbeen Region</rdfs:label>
    </owl:NamedIndividual>
    


    <!-- http://purl.obolibrary.org/obo/GAZ_00030912 -->

    <owl:NamedIndividual rdf:about="http://purl.obolibrary.org/obo/GAZ_00030912">
        <obo:RO_0001025 rdf:resource="http://purl.obolibrary.org/obo/GAZ_00000656"/>
        <obo:IAO_0000115>An administrative region (markaz) of Dakahlia Governorate.</obo:IAO_0000115>
        <oboInOwl:hasOBONamespace>GAZ</oboInOwl:hasOBONamespace>
        <oboInOwl:id>GAZ:00030912</oboInOwl:id>
        <rdfs:label>Talkha Region</rdfs:label>
    </owl:NamedIndividual>
    


    <!-- http://purl.obolibrary.org/obo/GAZ_00030913 -->

    <owl:NamedIndividual rdf:about="http://purl.obolibrary.org/obo/GAZ_00030913">
        <obo:RO_0001025 rdf:resource="http://purl.obolibrary.org/obo/GAZ_00000656"/>
        <obo:IAO_0000115>An administrative region (markaz) of Dakahlia Governorate.</obo:IAO_0000115>
        <oboInOwl:hasOBONamespace>GAZ</oboInOwl:hasOBONamespace>
        <oboInOwl:id>GAZ:00030913</oboInOwl:id>
        <rdfs:label>Meit Ghamr Region</rdfs:label>
    </owl:NamedIndividual>
    


    <!-- http://purl.obolibrary.org/obo/GAZ_00030914 -->

    <owl:NamedIndividual rdf:about="http://purl.obolibrary.org/obo/GAZ_00030914">
        <obo:RO_0001025 rdf:resource="http://purl.obolibrary.org/obo/GAZ_00000657"/>
        <obo:IAO_0000115>An administrative region (markaz) of Damietta Governorate.</obo:IAO_0000115>
        <oboInOwl:hasOBONamespace>GAZ</oboInOwl:hasOBONamespace>
        <oboInOwl:id>GAZ:00030914</oboInOwl:id>
        <rdfs:label>Faraskur Central Region</rdfs:label>
    </owl:NamedIndividual>
    


    <!-- http://purl.obolibrary.org/obo/GAZ_00030915 -->

    <owl:NamedIndividual rdf:about="http://purl.obolibrary.org/obo/GAZ_00030915">
        <obo:RO_0001025 rdf:resource="http://purl.obolibrary.org/obo/GAZ_00000657"/>
        <obo:IAO_0000115>An administrative region (markaz) of Damietta Governorate.</obo:IAO_0000115>
        <oboInOwl:hasOBONamespace>GAZ</oboInOwl:hasOBONamespace>
        <oboInOwl:id>GAZ:00030915</oboInOwl:id>
        <rdfs:label>Zarqa Central Region</rdfs:label>
    </owl:NamedIndividual>
    


    <!-- http://purl.obolibrary.org/obo/GAZ_00030916 -->

    <owl:NamedIndividual rdf:about="http://purl.obolibrary.org/obo/GAZ_00030916">
        <obo:RO_0001025 rdf:resource="http://purl.obolibrary.org/obo/GAZ_00000657"/>
        <obo:IAO_0000115>An administrative region (markaz) of Damietta Governorate.</obo:IAO_0000115>
        <oboInOwl:hasOBONamespace>GAZ</oboInOwl:hasOBONamespace>
        <oboInOwl:id>GAZ:00030916</oboInOwl:id>
        <rdfs:label>Kafr Saad Central Region</rdfs:label>
    </owl:NamedIndividual>
    


    <!-- http://purl.obolibrary.org/obo/GAZ_00030917 -->

    <owl:NamedIndividual rdf:about="http://purl.obolibrary.org/obo/GAZ_00030917">
        <obo:RO_0001025 rdf:resource="http://purl.obolibrary.org/obo/GAZ_00000657"/>
        <obo:IAO_0000115>An administrative region (markaz) of Damietta Governorate.</obo:IAO_0000115>
        <oboInOwl:hasOBONamespace>GAZ</oboInOwl:hasOBONamespace>
        <oboInOwl:id>GAZ:00030917</oboInOwl:id>
        <rdfs:label>Damietta Central Region</rdfs:label>
    </owl:NamedIndividual>
    


    <!-- http://purl.obolibrary.org/obo/GAZ_00030918 -->

    <owl:NamedIndividual rdf:about="http://purl.obolibrary.org/obo/GAZ_00030918">
        <obo:RO_0001025 rdf:resource="http://purl.obolibrary.org/obo/GAZ_00000660"/>
        <obo:IAO_0000115>An administrative region (markaz) of Monufia Governorate.</obo:IAO_0000115>
        <oboInOwl:hasOBONamespace>GAZ</oboInOwl:hasOBONamespace>
        <oboInOwl:id>GAZ:00030918</oboInOwl:id>
        <rdfs:label>Tala Region</rdfs:label>
    </owl:NamedIndividual>
    


    <!-- http://purl.obolibrary.org/obo/GAZ_00030919 -->

    <owl:NamedIndividual rdf:about="http://purl.obolibrary.org/obo/GAZ_00030919">
        <obo:RO_0001025 rdf:resource="http://purl.obolibrary.org/obo/GAZ_00000660"/>
        <obo:IAO_0000115>An administrative region (markaz) of Monufia Governorate.</obo:IAO_0000115>
        <oboInOwl:hasOBONamespace>GAZ</oboInOwl:hasOBONamespace>
        <oboInOwl:id>GAZ:00030919</oboInOwl:id>
        <rdfs:label>Menouf Region</rdfs:label>
    </owl:NamedIndividual>
    


    <!-- http://purl.obolibrary.org/obo/GAZ_00030920 -->

    <owl:NamedIndividual rdf:about="http://purl.obolibrary.org/obo/GAZ_00030920">
        <obo:RO_0001025 rdf:resource="http://purl.obolibrary.org/obo/GAZ_00000660"/>
        <obo:IAO_0000115>An administrative region (markaz) of Monufia Governorate.</obo:IAO_0000115>
        <oboInOwl:hasOBONamespace>GAZ</oboInOwl:hasOBONamespace>
        <oboInOwl:id>GAZ:00030920</oboInOwl:id>
        <rdfs:label>Ashmoon Region</rdfs:label>
    </owl:NamedIndividual>
    


    <!-- http://purl.obolibrary.org/obo/GAZ_00030921 -->

    <owl:NamedIndividual rdf:about="http://purl.obolibrary.org/obo/GAZ_00030921">
        <obo:RO_0001025 rdf:resource="http://purl.obolibrary.org/obo/GAZ_00000660"/>
        <obo:IAO_0000115>An administrative region (markaz) of Monufia Governorate.</obo:IAO_0000115>
        <oboInOwl:hasOBONamespace>GAZ</oboInOwl:hasOBONamespace>
        <oboInOwl:id>GAZ:00030921</oboInOwl:id>
        <rdfs:label>Al Bagoor Region</rdfs:label>
    </owl:NamedIndividual>
    


    <!-- http://purl.obolibrary.org/obo/GAZ_00030922 -->

    <owl:NamedIndividual rdf:about="http://purl.obolibrary.org/obo/GAZ_00030922">
        <obo:RO_0001025 rdf:resource="http://purl.obolibrary.org/obo/GAZ_00000660"/>
        <obo:IAO_0000115>An administrative region (markaz) of Monufia Governorate.</obo:IAO_0000115>
        <oboInOwl:hasOBONamespace>GAZ</oboInOwl:hasOBONamespace>
        <oboInOwl:id>GAZ:00030922</oboInOwl:id>
        <rdfs:label>Quesnah Region</rdfs:label>
    </owl:NamedIndividual>
    


    <!-- http://purl.obolibrary.org/obo/GAZ_00030923 -->

    <owl:NamedIndividual rdf:about="http://purl.obolibrary.org/obo/GAZ_00030923">
        <obo:RO_0001025 rdf:resource="http://purl.obolibrary.org/obo/GAZ_00000660"/>
        <obo:IAO_0000115>An administrative region (markaz) of Monufia Governorate.</obo:IAO_0000115>
        <oboInOwl:hasOBONamespace>GAZ</oboInOwl:hasOBONamespace>
        <oboInOwl:id>GAZ:00030923</oboInOwl:id>
        <rdfs:label>Al Shohadaa Region</rdfs:label>
    </owl:NamedIndividual>
    


    <!-- http://purl.obolibrary.org/obo/GAZ_00030924 -->

    <owl:NamedIndividual rdf:about="http://purl.obolibrary.org/obo/GAZ_00030924">
        <obo:RO_0001025 rdf:resource="http://purl.obolibrary.org/obo/GAZ_00000660"/>
        <obo:IAO_0000115>An administrative region (kism) of Monufia Governorate.</obo:IAO_0000115>
        <oboInOwl:hasOBONamespace>GAZ</oboInOwl:hasOBONamespace>
        <oboInOwl:id>GAZ:00030924</oboInOwl:id>
        <rdfs:label>Kism Sirs al Layyanah</rdfs:label>
    </owl:NamedIndividual>
    


    <!-- http://purl.obolibrary.org/obo/GAZ_00030925 -->

    <owl:NamedIndividual rdf:about="http://purl.obolibrary.org/obo/GAZ_00030925">
        <obo:RO_0001025 rdf:resource="http://purl.obolibrary.org/obo/GAZ_00000660"/>
        <obo:IAO_0000115>An administrative region (markaz) of Monufia Governorate.</obo:IAO_0000115>
        <oboInOwl:hasOBONamespace>GAZ</oboInOwl:hasOBONamespace>
        <oboInOwl:id>GAZ:00030925</oboInOwl:id>
        <rdfs:label>Berkat Al Sabaa Region</rdfs:label>
    </owl:NamedIndividual>
    


    <!-- http://purl.obolibrary.org/obo/GAZ_00030926 -->

    <owl:NamedIndividual rdf:about="http://purl.obolibrary.org/obo/GAZ_00030926">
        <obo:RO_0001025 rdf:resource="http://purl.obolibrary.org/obo/GAZ_00000660"/>
        <obo:IAO_0000115>An administrative region (markaz) of Monufia Governorate.</obo:IAO_0000115>
        <oboInOwl:hasOBONamespace>GAZ</oboInOwl:hasOBONamespace>
        <oboInOwl:id>GAZ:00030926</oboInOwl:id>
        <rdfs:label>Al Sadat Region</rdfs:label>
    </owl:NamedIndividual>
    


    <!-- http://purl.obolibrary.org/obo/GAZ_00030927 -->

    <owl:NamedIndividual rdf:about="http://purl.obolibrary.org/obo/GAZ_00030927">
        <obo:RO_0001025 rdf:resource="http://purl.obolibrary.org/obo/GAZ_00000660"/>
        <obo:IAO_0000115>An administrative region (markaz) of Monufia Governorate.</obo:IAO_0000115>
        <oboInOwl:hasOBONamespace>GAZ</oboInOwl:hasOBONamespace>
        <oboInOwl:id>GAZ:00030927</oboInOwl:id>
        <rdfs:label>Shebeen El Koom Region</rdfs:label>
    </owl:NamedIndividual>
    


    <!-- http://purl.obolibrary.org/obo/GAZ_00030928 -->

    <owl:NamedIndividual rdf:about="http://purl.obolibrary.org/obo/GAZ_00030928">
        <obo:RO_0001025 rdf:resource="http://purl.obolibrary.org/obo/GAZ_00000652"/>
        <obo:IAO_0000115>An administrative region (markaz) of Sohag Governorate.</obo:IAO_0000115>
        <oboInOwl:hasOBONamespace>GAZ</oboInOwl:hasOBONamespace>
        <oboInOwl:id>GAZ:00030928</oboInOwl:id>
        <rdfs:label>Sakulta Region</rdfs:label>
    </owl:NamedIndividual>
    


    <!-- http://purl.obolibrary.org/obo/GAZ_00030929 -->

    <owl:NamedIndividual rdf:about="http://purl.obolibrary.org/obo/GAZ_00030929">
        <obo:RO_0001025 rdf:resource="http://purl.obolibrary.org/obo/GAZ_00000652"/>
        <obo:IAO_0000115>An administrative region (markaz) of Sohag Governorate.</obo:IAO_0000115>
        <oboInOwl:hasOBONamespace>GAZ</oboInOwl:hasOBONamespace>
        <oboInOwl:id>GAZ:00030929</oboInOwl:id>
        <rdfs:label>Tahta Region</rdfs:label>
    </owl:NamedIndividual>
    


    <!-- http://purl.obolibrary.org/obo/GAZ_00030930 -->

    <owl:NamedIndividual rdf:about="http://purl.obolibrary.org/obo/GAZ_00030930">
        <obo:RO_0001025 rdf:resource="http://purl.obolibrary.org/obo/GAZ_00000652"/>
        <obo:IAO_0000115>An administrative region (markaz) of Sohag Governorate.</obo:IAO_0000115>
        <oboInOwl:hasOBONamespace>GAZ</oboInOwl:hasOBONamespace>
        <oboInOwl:id>GAZ:00030930</oboInOwl:id>
        <rdfs:label>el-Balyana Region</rdfs:label>
    </owl:NamedIndividual>
    


    <!-- http://purl.obolibrary.org/obo/GAZ_00030931 -->

    <owl:NamedIndividual rdf:about="http://purl.obolibrary.org/obo/GAZ_00030931">
        <obo:RO_0001025 rdf:resource="http://purl.obolibrary.org/obo/GAZ_00000652"/>
        <obo:IAO_0000115>An administrative region (markaz) of Sohag Governorate.</obo:IAO_0000115>
        <oboInOwl:hasOBONamespace>GAZ</oboInOwl:hasOBONamespace>
        <oboInOwl:id>GAZ:00030931</oboInOwl:id>
        <rdfs:label>Akhmim Region</rdfs:label>
    </owl:NamedIndividual>
    


    <!-- http://purl.obolibrary.org/obo/GAZ_00030932 -->

    <owl:NamedIndividual rdf:about="http://purl.obolibrary.org/obo/GAZ_00030932">
        <obo:RO_0001025 rdf:resource="http://purl.obolibrary.org/obo/GAZ_00000652"/>
        <obo:IAO_0000115>An administrative region (markaz) of Sohag Governorate.</obo:IAO_0000115>
        <oboInOwl:hasOBONamespace>GAZ</oboInOwl:hasOBONamespace>
        <oboInOwl:id>GAZ:00030932</oboInOwl:id>
        <rdfs:label>Dar el-Salam Region</rdfs:label>
    </owl:NamedIndividual>
    


    <!-- http://purl.obolibrary.org/obo/GAZ_00030933 -->

    <owl:NamedIndividual rdf:about="http://purl.obolibrary.org/obo/GAZ_00030933">
        <obo:RO_0001025 rdf:resource="http://purl.obolibrary.org/obo/GAZ_00000652"/>
        <obo:IAO_0000115>An administrative region (markaz) of Sohag Governorate.</obo:IAO_0000115>
        <oboInOwl:hasOBONamespace>GAZ</oboInOwl:hasOBONamespace>
        <oboInOwl:id>GAZ:00030933</oboInOwl:id>
        <rdfs:label>Sohag Region</rdfs:label>
    </owl:NamedIndividual>
    


    <!-- http://purl.obolibrary.org/obo/GAZ_00030934 -->

    <owl:NamedIndividual rdf:about="http://purl.obolibrary.org/obo/GAZ_00030934">
        <obo:RO_0001025 rdf:resource="http://purl.obolibrary.org/obo/GAZ_00000652"/>
        <obo:IAO_0000115>An administrative region (markaz) of Sohag Governorate.</obo:IAO_0000115>
        <oboInOwl:hasOBONamespace>GAZ</oboInOwl:hasOBONamespace>
        <oboInOwl:id>GAZ:00030934</oboInOwl:id>
        <rdfs:label>el-Mansha Region</rdfs:label>
    </owl:NamedIndividual>
    


    <!-- http://purl.obolibrary.org/obo/GAZ_00030935 -->

    <owl:NamedIndividual rdf:about="http://purl.obolibrary.org/obo/GAZ_00030935">
        <obo:RO_0001025 rdf:resource="http://purl.obolibrary.org/obo/GAZ_00000652"/>
        <obo:IAO_0000115>An administrative region (markaz) of Sohag Governorate.</obo:IAO_0000115>
        <oboInOwl:hasOBONamespace>GAZ</oboInOwl:hasOBONamespace>
        <oboInOwl:id>GAZ:00030935</oboInOwl:id>
        <rdfs:label>Tima Region</rdfs:label>
    </owl:NamedIndividual>
    


    <!-- http://purl.obolibrary.org/obo/GAZ_00030936 -->

    <owl:NamedIndividual rdf:about="http://purl.obolibrary.org/obo/GAZ_00030936">
        <obo:RO_0001025 rdf:resource="http://purl.obolibrary.org/obo/GAZ_00000652"/>
        <obo:IAO_0000115>An administrative region (markaz) of Sohag Governorate.</obo:IAO_0000115>
        <oboInOwl:hasOBONamespace>GAZ</oboInOwl:hasOBONamespace>
        <oboInOwl:id>GAZ:00030936</oboInOwl:id>
        <rdfs:label>Girga Region</rdfs:label>
    </owl:NamedIndividual>
    


    <!-- http://purl.obolibrary.org/obo/GAZ_00030937 -->

    <owl:NamedIndividual rdf:about="http://purl.obolibrary.org/obo/GAZ_00030937">
        <obo:RO_0001025 rdf:resource="http://purl.obolibrary.org/obo/GAZ_00000652"/>
        <obo:IAO_0000115>An administrative region (markaz) of Sohag Governorate.</obo:IAO_0000115>
        <oboInOwl:hasOBONamespace>GAZ</oboInOwl:hasOBONamespace>
        <oboInOwl:id>GAZ:00030937</oboInOwl:id>
        <rdfs:label>el-Usayrat Region</rdfs:label>
    </owl:NamedIndividual>
    


    <!-- http://purl.obolibrary.org/obo/GAZ_00030938 -->

    <owl:NamedIndividual rdf:about="http://purl.obolibrary.org/obo/GAZ_00030938">
        <obo:RO_0001025 rdf:resource="http://purl.obolibrary.org/obo/GAZ_00000652"/>
        <obo:IAO_0000115>An administrative region (markaz) of Sohag Governorate.</obo:IAO_0000115>
        <oboInOwl:hasOBONamespace>GAZ</oboInOwl:hasOBONamespace>
        <oboInOwl:id>GAZ:00030938</oboInOwl:id>
        <rdfs:label>Juhayna Region</rdfs:label>
    </owl:NamedIndividual>
    


    <!-- http://purl.obolibrary.org/obo/GAZ_00030939 -->

    <owl:NamedIndividual rdf:about="http://purl.obolibrary.org/obo/GAZ_00030939">
        <obo:RO_0001025 rdf:resource="http://purl.obolibrary.org/obo/GAZ_00000652"/>
        <obo:IAO_0000115>An administrative region (markaz) of Sohag Governorate.</obo:IAO_0000115>
        <oboInOwl:hasOBONamespace>GAZ</oboInOwl:hasOBONamespace>
        <oboInOwl:id>GAZ:00030939</oboInOwl:id>
        <rdfs:label>el-Maragha Region</rdfs:label>
    </owl:NamedIndividual>
    


    <!-- http://purl.obolibrary.org/obo/GAZ_00030940 -->

    <owl:NamedIndividual rdf:about="http://purl.obolibrary.org/obo/GAZ_00030940">
        <obo:RO_0001025 rdf:resource="http://purl.obolibrary.org/obo/GAZ_00000649"/>
        <oboInOwl:hasOBONamespace>GAZ</oboInOwl:hasOBONamespace>
        <oboInOwl:id>GAZ:00030940</oboInOwl:id>
        <rdfs:label>Giza Region</rdfs:label>
    </owl:NamedIndividual>
    


    <!-- http://purl.obolibrary.org/obo/GAZ_00030941 -->

    <owl:NamedIndividual rdf:about="http://purl.obolibrary.org/obo/GAZ_00030941">
        <obo:RO_0001025 rdf:resource="http://purl.obolibrary.org/obo/GAZ_00000649"/>
        <obo:IAO_0000115>An administrative region (markaz) of Giza Governorate.</obo:IAO_0000115>
        <oboInOwl:hasOBONamespace>GAZ</oboInOwl:hasOBONamespace>
        <oboInOwl:id>GAZ:00030941</oboInOwl:id>
        <rdfs:label>Atfih Region</rdfs:label>
    </owl:NamedIndividual>
    


    <!-- http://purl.obolibrary.org/obo/GAZ_00030946 -->

    <owl:NamedIndividual rdf:about="http://purl.obolibrary.org/obo/GAZ_00030946">
        <obo:RO_0001025 rdf:resource="http://purl.obolibrary.org/obo/GAZ_00000649"/>
        <obo:IAO_0000115>An administrative region (markaz) of Giza Governorate.</obo:IAO_0000115>
        <oboInOwl:hasOBONamespace>GAZ</oboInOwl:hasOBONamespace>
        <oboInOwl:id>GAZ:00030946</oboInOwl:id>
        <rdfs:label>Al-Saff Region</rdfs:label>
    </owl:NamedIndividual>
    


    <!-- http://purl.obolibrary.org/obo/GAZ_00030947 -->

    <owl:NamedIndividual rdf:about="http://purl.obolibrary.org/obo/GAZ_00030947">
        <obo:RO_0001025 rdf:resource="http://purl.obolibrary.org/obo/GAZ_00000649"/>
        <obo:IAO_0000115>An administrative region (markaz) of Giza Governorate.</obo:IAO_0000115>
        <oboInOwl:hasOBONamespace>GAZ</oboInOwl:hasOBONamespace>
        <oboInOwl:id>GAZ:00030947</oboInOwl:id>
        <rdfs:label>Aoseem Region</rdfs:label>
    </owl:NamedIndividual>
    


    <!-- http://purl.obolibrary.org/obo/GAZ_00030948 -->

    <owl:NamedIndividual rdf:about="http://purl.obolibrary.org/obo/GAZ_00030948">
        <obo:RO_0001025 rdf:resource="http://purl.obolibrary.org/obo/GAZ_00000649"/>
        <obo:IAO_0000115>An administrative region (markaz) of Giza Governorate.</obo:IAO_0000115>
        <oboInOwl:hasOBONamespace>GAZ</oboInOwl:hasOBONamespace>
        <oboInOwl:id>GAZ:00030948</oboInOwl:id>
        <rdfs:label>Al-Bdrasheen</rdfs:label>
    </owl:NamedIndividual>
    


    <!-- http://purl.obolibrary.org/obo/GAZ_00030949 -->

    <owl:NamedIndividual rdf:about="http://purl.obolibrary.org/obo/GAZ_00030949">
        <obo:RO_0001025 rdf:resource="http://purl.obolibrary.org/obo/GAZ_00000649"/>
        <obo:IAO_0000115>An administrative region (markaz) of Giza Governorate.</obo:IAO_0000115>
        <oboInOwl:hasOBONamespace>GAZ</oboInOwl:hasOBONamespace>
        <oboInOwl:id>GAZ:00030949</oboInOwl:id>
        <rdfs:label>Al-Aiat Region</rdfs:label>
    </owl:NamedIndividual>
    


    <!-- http://purl.obolibrary.org/obo/GAZ_00030950 -->

    <owl:NamedIndividual rdf:about="http://purl.obolibrary.org/obo/GAZ_00030950">
        <obo:RO_0001025 rdf:resource="http://purl.obolibrary.org/obo/GAZ_00000651"/>
        <oboInOwl:hasOBONamespace>GAZ</oboInOwl:hasOBONamespace>
        <oboInOwl:id>GAZ:00030950</oboInOwl:id>
        <rdfs:label>Nag Hammadi Region</rdfs:label>
    </owl:NamedIndividual>
    


    <!-- http://purl.obolibrary.org/obo/GAZ_00030951 -->

    <owl:NamedIndividual rdf:about="http://purl.obolibrary.org/obo/GAZ_00030951">
        <obo:RO_0001025 rdf:resource="http://purl.obolibrary.org/obo/GAZ_00000651"/>
        <obo:IAO_0000115>An administrative region (markaz) of Qena Governorate.</obo:IAO_0000115>
        <oboInOwl:hasOBONamespace>GAZ</oboInOwl:hasOBONamespace>
        <oboInOwl:id>GAZ:00030951</oboInOwl:id>
        <rdfs:label>Deshna Region</rdfs:label>
    </owl:NamedIndividual>
    


    <!-- http://purl.obolibrary.org/obo/GAZ_00030952 -->

    <owl:NamedIndividual rdf:about="http://purl.obolibrary.org/obo/GAZ_00030952">
        <obo:RO_0001025 rdf:resource="http://purl.obolibrary.org/obo/GAZ_00066402"/>
        <oboInOwl:hasOBONamespace>GAZ</oboInOwl:hasOBONamespace>
        <oboInOwl:id>GAZ:00030952</oboInOwl:id>
        <rdfs:label>Luxor City</rdfs:label>
    </owl:NamedIndividual>
    


    <!-- http://purl.obolibrary.org/obo/GAZ_00030953 -->

    <owl:NamedIndividual rdf:about="http://purl.obolibrary.org/obo/GAZ_00030953">
        <obo:RO_0001025 rdf:resource="http://purl.obolibrary.org/obo/GAZ_00000651"/>
        <obo:IAO_0000115>An administrative region (markaz) of Qena Governorate.</obo:IAO_0000115>
        <oboInOwl:hasOBONamespace>GAZ</oboInOwl:hasOBONamespace>
        <oboInOwl:id>GAZ:00030953</oboInOwl:id>
        <rdfs:label>Naqada Region</rdfs:label>
    </owl:NamedIndividual>
    


    <!-- http://purl.obolibrary.org/obo/GAZ_00030954 -->

    <owl:NamedIndividual rdf:about="http://purl.obolibrary.org/obo/GAZ_00030954">
        <obo:RO_0001025 rdf:resource="http://purl.obolibrary.org/obo/GAZ_00000651"/>
        <obo:IAO_0000115>An administrative region (markaz) of Qena Governorate.</obo:IAO_0000115>
        <oboInOwl:hasOBONamespace>GAZ</oboInOwl:hasOBONamespace>
        <oboInOwl:id>GAZ:00030954</oboInOwl:id>
        <rdfs:label>Abu Tesht Region</rdfs:label>
    </owl:NamedIndividual>
    


    <!-- http://purl.obolibrary.org/obo/GAZ_00030955 -->

    <owl:NamedIndividual rdf:about="http://purl.obolibrary.org/obo/GAZ_00030955">
        <obo:RO_0001025 rdf:resource="http://purl.obolibrary.org/obo/GAZ_00000651"/>
        <obo:IAO_0000115>An administrative region (markaz) of Qena Governorate.</obo:IAO_0000115>
        <oboInOwl:hasOBONamespace>GAZ</oboInOwl:hasOBONamespace>
        <oboInOwl:id>GAZ:00030955</oboInOwl:id>
        <rdfs:label>Qift Region</rdfs:label>
    </owl:NamedIndividual>
    


    <!-- http://purl.obolibrary.org/obo/GAZ_00030956 -->

    <owl:NamedIndividual rdf:about="http://purl.obolibrary.org/obo/GAZ_00030956">
        <obo:RO_0001025 rdf:resource="http://purl.obolibrary.org/obo/GAZ_00000651"/>
        <obo:IAO_0000115>An administrative region (markaz) of Qena Governorate.</obo:IAO_0000115>
        <oboInOwl:hasOBONamespace>GAZ</oboInOwl:hasOBONamespace>
        <oboInOwl:id>GAZ:00030956</oboInOwl:id>
        <rdfs:label>Armant Region</rdfs:label>
    </owl:NamedIndividual>
    


    <!-- http://purl.obolibrary.org/obo/GAZ_00030957 -->

    <owl:NamedIndividual rdf:about="http://purl.obolibrary.org/obo/GAZ_00030957">
        <obo:RO_0001025 rdf:resource="http://purl.obolibrary.org/obo/GAZ_00000651"/>
        <obo:IAO_0000115>An administrative region (markaz) of Qena Governorate.</obo:IAO_0000115>
        <oboInOwl:hasOBONamespace>GAZ</oboInOwl:hasOBONamespace>
        <oboInOwl:id>GAZ:00030957</oboInOwl:id>
        <rdfs:label>Qena Region</rdfs:label>
    </owl:NamedIndividual>
    


    <!-- http://purl.obolibrary.org/obo/GAZ_00030958 -->

    <owl:NamedIndividual rdf:about="http://purl.obolibrary.org/obo/GAZ_00030958">
        <obo:RO_0001025 rdf:resource="http://purl.obolibrary.org/obo/GAZ_00000651"/>
        <obo:IAO_0000115>An administrative region (markaz) of Qena Governorate.</obo:IAO_0000115>
        <oboInOwl:hasOBONamespace>GAZ</oboInOwl:hasOBONamespace>
        <oboInOwl:id>GAZ:00030958</oboInOwl:id>
        <rdfs:label>El Wakf Region</rdfs:label>
    </owl:NamedIndividual>
    


    <!-- http://purl.obolibrary.org/obo/GAZ_00030959 -->

    <owl:NamedIndividual rdf:about="http://purl.obolibrary.org/obo/GAZ_00030959">
        <obo:RO_0001025 rdf:resource="http://purl.obolibrary.org/obo/GAZ_00000651"/>
        <obo:IAO_0000115>An administrative region (markaz) of Qena Governorate.</obo:IAO_0000115>
        <oboInOwl:hasOBONamespace>GAZ</oboInOwl:hasOBONamespace>
        <oboInOwl:id>GAZ:00030959</oboInOwl:id>
        <rdfs:label>Esna Region</rdfs:label>
    </owl:NamedIndividual>
    


    <!-- http://purl.obolibrary.org/obo/GAZ_00030960 -->

    <owl:NamedIndividual rdf:about="http://purl.obolibrary.org/obo/GAZ_00030960">
        <obo:RO_0001025 rdf:resource="http://purl.obolibrary.org/obo/GAZ_00000651"/>
        <obo:IAO_0000115>An administrative region (markaz) of Qena Governorate.</obo:IAO_0000115>
        <oboInOwl:hasOBONamespace>GAZ</oboInOwl:hasOBONamespace>
        <oboInOwl:id>GAZ:00030960</oboInOwl:id>
        <rdfs:label>Farshout Region</rdfs:label>
    </owl:NamedIndividual>
    


    <!-- http://purl.obolibrary.org/obo/GAZ_00030961 -->

    <owl:NamedIndividual rdf:about="http://purl.obolibrary.org/obo/GAZ_00030961">
        <obo:RO_0001025 rdf:resource="http://purl.obolibrary.org/obo/GAZ_00000651"/>
        <obo:IAO_0000115>An administrative region (markaz) of Qena Governorate.</obo:IAO_0000115>
        <oboInOwl:hasOBONamespace>GAZ</oboInOwl:hasOBONamespace>
        <oboInOwl:id>GAZ:00030961</oboInOwl:id>
        <rdfs:label>Qus Region</rdfs:label>
    </owl:NamedIndividual>
    


    <!-- http://purl.obolibrary.org/obo/GAZ_00030962 -->

    <owl:NamedIndividual rdf:about="http://purl.obolibrary.org/obo/GAZ_00030962">
        <obo:RO_0001025 rdf:resource="http://purl.obolibrary.org/obo/GAZ_00000659"/>
        <obo:IAO_0000115>An administrative region (markaz) of Kafr el-Sheikh Governorate.</obo:IAO_0000115>
        <oboInOwl:hasOBONamespace>GAZ</oboInOwl:hasOBONamespace>
        <oboInOwl:id>GAZ:00030962</oboInOwl:id>
        <rdfs:label>Beila Region</rdfs:label>
    </owl:NamedIndividual>
    


    <!-- http://purl.obolibrary.org/obo/GAZ_00030963 -->

    <owl:NamedIndividual rdf:about="http://purl.obolibrary.org/obo/GAZ_00030963">
        <obo:RO_0001025 rdf:resource="http://purl.obolibrary.org/obo/GAZ_00000659"/>
        <obo:IAO_0000115>An administrative region (markaz) of Kafr el-Sheikh Governorate.</obo:IAO_0000115>
        <oboInOwl:hasOBONamespace>GAZ</oboInOwl:hasOBONamespace>
        <oboInOwl:id>GAZ:00030963</oboInOwl:id>
        <rdfs:label>Al Riad Region</rdfs:label>
    </owl:NamedIndividual>
    


    <!-- http://purl.obolibrary.org/obo/GAZ_00030964 -->

    <owl:NamedIndividual rdf:about="http://purl.obolibrary.org/obo/GAZ_00030964">
        <obo:RO_0001025 rdf:resource="http://purl.obolibrary.org/obo/GAZ_00000659"/>
        <obo:IAO_0000115>An administrative region (markaz) of Kafr el-Sheikh Governorate.</obo:IAO_0000115>
        <oboInOwl:hasOBONamespace>GAZ</oboInOwl:hasOBONamespace>
        <oboInOwl:id>GAZ:00030964</oboInOwl:id>
        <rdfs:label>Desouk Region</rdfs:label>
    </owl:NamedIndividual>
    


    <!-- http://purl.obolibrary.org/obo/GAZ_00030965 -->

    <owl:NamedIndividual rdf:about="http://purl.obolibrary.org/obo/GAZ_00030965">
        <obo:RO_0001025 rdf:resource="http://purl.obolibrary.org/obo/GAZ_00000659"/>
        <obo:IAO_0000115>An administrative region (markaz) of Kafr el-Sheikh Governorate.</obo:IAO_0000115>
        <oboInOwl:hasOBONamespace>GAZ</oboInOwl:hasOBONamespace>
        <oboInOwl:id>GAZ:00030965</oboInOwl:id>
        <rdfs:label>Foah Region</rdfs:label>
    </owl:NamedIndividual>
    


    <!-- http://purl.obolibrary.org/obo/GAZ_00030966 -->

    <owl:NamedIndividual rdf:about="http://purl.obolibrary.org/obo/GAZ_00030966">
        <obo:RO_0001025 rdf:resource="http://purl.obolibrary.org/obo/GAZ_00000659"/>
        <obo:IAO_0000115>An administrative region (markaz) of Kafr el-Sheikh Governorate.</obo:IAO_0000115>
        <oboInOwl:hasOBONamespace>GAZ</oboInOwl:hasOBONamespace>
        <oboInOwl:id>GAZ:00030966</oboInOwl:id>
        <rdfs:label>Kafr el-Sheikh Region</rdfs:label>
    </owl:NamedIndividual>
    


    <!-- http://purl.obolibrary.org/obo/GAZ_00030967 -->

    <owl:NamedIndividual rdf:about="http://purl.obolibrary.org/obo/GAZ_00030967">
        <obo:RO_0001025 rdf:resource="http://purl.obolibrary.org/obo/GAZ_00000659"/>
        <obo:IAO_0000115>An administrative region (markaz) of Kafr el-Sheikh Governorate.</obo:IAO_0000115>
        <oboInOwl:hasOBONamespace>GAZ</oboInOwl:hasOBONamespace>
        <oboInOwl:id>GAZ:00030967</oboInOwl:id>
        <rdfs:label>Al Hamool Region</rdfs:label>
    </owl:NamedIndividual>
    


    <!-- http://purl.obolibrary.org/obo/GAZ_00030968 -->

    <owl:NamedIndividual rdf:about="http://purl.obolibrary.org/obo/GAZ_00030968">
        <obo:RO_0001025 rdf:resource="http://purl.obolibrary.org/obo/GAZ_00000659"/>
        <obo:IAO_0000115>A populated place. A resort in Kafr el-Sheikh Governorate, in the north of Egypt.</obo:IAO_0000115>
        <oboInOwl:hasOBONamespace>GAZ</oboInOwl:hasOBONamespace>
        <oboInOwl:id>GAZ:00030968</oboInOwl:id>
        <rdfs:label>Balteem</rdfs:label>
    </owl:NamedIndividual>
    


    <!-- http://purl.obolibrary.org/obo/GAZ_00030969 -->

    <owl:NamedIndividual rdf:about="http://purl.obolibrary.org/obo/GAZ_00030969">
        <obo:RO_0001025 rdf:resource="http://purl.obolibrary.org/obo/GAZ_00000659"/>
        <obo:IAO_0000115>An administrative region (markaz) of Kafr el-Sheikh Governorate.</obo:IAO_0000115>
        <oboInOwl:hasOBONamespace>GAZ</oboInOwl:hasOBONamespace>
        <oboInOwl:id>GAZ:00030969</oboInOwl:id>
        <rdfs:label>Metobas Region</rdfs:label>
    </owl:NamedIndividual>
    


    <!-- http://purl.obolibrary.org/obo/GAZ_00030970 -->

    <owl:NamedIndividual rdf:about="http://purl.obolibrary.org/obo/GAZ_00030970">
        <obo:RO_0001025 rdf:resource="http://purl.obolibrary.org/obo/GAZ_00000659"/>
        <obo:IAO_0000115>An administrative region (markaz) of Kafr el-Sheikh Governorate.</obo:IAO_0000115>
        <oboInOwl:hasOBONamespace>GAZ</oboInOwl:hasOBONamespace>
        <oboInOwl:id>GAZ:00030970</oboInOwl:id>
        <rdfs:label>Kellien Region</rdfs:label>
    </owl:NamedIndividual>
    


    <!-- http://purl.obolibrary.org/obo/GAZ_00030971 -->

    <owl:NamedIndividual rdf:about="http://purl.obolibrary.org/obo/GAZ_00030971">
        <obo:RO_0001025 rdf:resource="http://purl.obolibrary.org/obo/GAZ_00000659"/>
        <obo:IAO_0000115>An administrative region (markaz) of Kafr el-Sheikh Governorate.</obo:IAO_0000115>
        <oboInOwl:hasOBONamespace>GAZ</oboInOwl:hasOBONamespace>
        <oboInOwl:id>GAZ:00030971</oboInOwl:id>
        <rdfs:label>Saiedy Region</rdfs:label>
    </owl:NamedIndividual>
    


    <!-- http://purl.obolibrary.org/obo/GAZ_00030972 -->

    <owl:NamedIndividual rdf:about="http://purl.obolibrary.org/obo/GAZ_00030972">
        <obo:RO_0001025 rdf:resource="http://purl.obolibrary.org/obo/GAZ_00000670"/>
        <obo:IAO_0000115>An administrative region (kism) of South Sinai Governorate.</obo:IAO_0000115>
        <oboInOwl:hasOBONamespace>GAZ</oboInOwl:hasOBONamespace>
        <oboInOwl:id>GAZ:00030972</oboInOwl:id>
        <rdfs:label>Kism Abu Zanimah</rdfs:label>
    </owl:NamedIndividual>
    


    <!-- http://purl.obolibrary.org/obo/GAZ_00030973 -->

    <owl:NamedIndividual rdf:about="http://purl.obolibrary.org/obo/GAZ_00030973">
        <obo:RO_0001025 rdf:resource="http://purl.obolibrary.org/obo/GAZ_00000670"/>
        <obo:IAO_0000115>An administrative region (kism) of South Sinai Governorate.</obo:IAO_0000115>
        <oboInOwl:hasOBONamespace>GAZ</oboInOwl:hasOBONamespace>
        <oboInOwl:id>GAZ:00030973</oboInOwl:id>
        <rdfs:label>Kism At Tur</rdfs:label>
    </owl:NamedIndividual>
    


    <!-- http://purl.obolibrary.org/obo/GAZ_00030974 -->

    <owl:NamedIndividual rdf:about="http://purl.obolibrary.org/obo/GAZ_00030974">
        <obo:RO_0001025 rdf:resource="http://purl.obolibrary.org/obo/GAZ_00000670"/>
        <obo:IAO_0000115>An administrative region (kism) of South Sinai Governorate.</obo:IAO_0000115>
        <oboInOwl:hasOBONamespace>GAZ</oboInOwl:hasOBONamespace>
        <oboInOwl:id>GAZ:00030974</oboInOwl:id>
        <rdfs:label>Kism Ras Sudr</rdfs:label>
    </owl:NamedIndividual>
    


    <!-- http://purl.obolibrary.org/obo/GAZ_00030975 -->

    <owl:NamedIndividual rdf:about="http://purl.obolibrary.org/obo/GAZ_00030975">
        <obo:RO_0001025 rdf:resource="http://purl.obolibrary.org/obo/GAZ_00000670"/>
        <obo:IAO_0000115>An administrative region (kism) of South Sinai Governorate.</obo:IAO_0000115>
        <oboInOwl:hasOBONamespace>GAZ</oboInOwl:hasOBONamespace>
        <oboInOwl:id>GAZ:00030975</oboInOwl:id>
        <rdfs:label>Kism Al Qiddisah Katrina</rdfs:label>
    </owl:NamedIndividual>
    


    <!-- http://purl.obolibrary.org/obo/GAZ_00030976 -->

    <owl:NamedIndividual rdf:about="http://purl.obolibrary.org/obo/GAZ_00030976">
        <obo:RO_0001025 rdf:resource="http://purl.obolibrary.org/obo/GAZ_00000670"/>
        <obo:IAO_0000115>An administrative region (kism) of South Sinai Governorate.</obo:IAO_0000115>
        <oboInOwl:hasOBONamespace>GAZ</oboInOwl:hasOBONamespace>
        <oboInOwl:id>GAZ:00030976</oboInOwl:id>
        <rdfs:label>Kism Sharm ash Shaykh</rdfs:label>
    </owl:NamedIndividual>
    


    <!-- http://purl.obolibrary.org/obo/GAZ_00030977 -->

    <owl:NamedIndividual rdf:about="http://purl.obolibrary.org/obo/GAZ_00030977">
        <obo:RO_0001025 rdf:resource="http://purl.obolibrary.org/obo/GAZ_00000670"/>
        <obo:IAO_0000115>An administrative region (kism) of South Sinai Governorate.</obo:IAO_0000115>
        <oboInOwl:hasOBONamespace>GAZ</oboInOwl:hasOBONamespace>
        <oboInOwl:id>GAZ:00030977</oboInOwl:id>
        <rdfs:label>Kism Abu Rudays</rdfs:label>
    </owl:NamedIndividual>
    


    <!-- http://purl.obolibrary.org/obo/GAZ_00030979 -->

    <owl:NamedIndividual rdf:about="http://purl.obolibrary.org/obo/GAZ_00030979">
        <obo:RO_0001025 rdf:resource="http://purl.obolibrary.org/obo/GAZ_00000670"/>
        <obo:IAO_0000115>An administrative region of South Sinai Governorate.</obo:IAO_0000115>
        <oboInOwl:hasOBONamespace>GAZ</oboInOwl:hasOBONamespace>
        <oboInOwl:id>GAZ:00030979</oboInOwl:id>
        <rdfs:label>Taba Region</rdfs:label>
    </owl:NamedIndividual>
    


    <!-- http://purl.obolibrary.org/obo/GAZ_00030980 -->

    <owl:NamedIndividual rdf:about="http://purl.obolibrary.org/obo/GAZ_00030980">
        <obo:RO_0001025 rdf:resource="http://purl.obolibrary.org/obo/GAZ_00000670"/>
        <obo:IAO_0000115>An administrative region (kism) of South Sinai Governorate.</obo:IAO_0000115>
        <oboInOwl:hasOBONamespace>GAZ</oboInOwl:hasOBONamespace>
        <oboInOwl:id>GAZ:00030980</oboInOwl:id>
        <rdfs:label>Kism Nuwaybi&apos;a</rdfs:label>
    </owl:NamedIndividual>
    


    <!-- http://purl.obolibrary.org/obo/GAZ_00030981 -->

    <owl:NamedIndividual rdf:about="http://purl.obolibrary.org/obo/GAZ_00030981">
        <obo:RO_0001025 rdf:resource="http://purl.obolibrary.org/obo/GAZ_00066411"/>
        <oboInOwl:hasOBONamespace>GAZ</oboInOwl:hasOBONamespace>
        <oboInOwl:id>GAZ:00030981</oboInOwl:id>
        <rdfs:label>Port Said</rdfs:label>
    </owl:NamedIndividual>
    


    <!-- http://purl.obolibrary.org/obo/GAZ_00030982 -->

    <owl:NamedIndividual rdf:about="http://purl.obolibrary.org/obo/GAZ_00030982">
        <rdf:type rdf:resource="http://purl.obolibrary.org/obo/ENVO_00000004"/>
        <obo:RO_0001025 rdf:resource="http://purl.obolibrary.org/obo/GAZ_00030981"/>
        <obo:IAO_0000115>A district of Port Said.</obo:IAO_0000115>
        <oboInOwl:hasOBONamespace>GAZ</oboInOwl:hasOBONamespace>
        <oboInOwl:id>GAZ:00030982</oboInOwl:id>
        <rdfs:label>Hai El Zhoohor</rdfs:label>
    </owl:NamedIndividual>
    


    <!-- http://purl.obolibrary.org/obo/GAZ_00030983 -->

    <owl:NamedIndividual rdf:about="http://purl.obolibrary.org/obo/GAZ_00030983">
        <rdf:type rdf:resource="http://purl.obolibrary.org/obo/ENVO_00000004"/>
        <obo:RO_0001025 rdf:resource="http://purl.obolibrary.org/obo/GAZ_00030981"/>
        <obo:IAO_0000115>A district of Port Said.</obo:IAO_0000115>
        <oboInOwl:hasOBONamespace>GAZ</oboInOwl:hasOBONamespace>
        <oboInOwl:id>GAZ:00030983</oboInOwl:id>
        <rdfs:label>Hai El Arab</rdfs:label>
    </owl:NamedIndividual>
    


    <!-- http://purl.obolibrary.org/obo/GAZ_00030984 -->

    <owl:NamedIndividual rdf:about="http://purl.obolibrary.org/obo/GAZ_00030984">
        <rdf:type rdf:resource="http://purl.obolibrary.org/obo/ENVO_00000004"/>
        <obo:RO_0001025 rdf:resource="http://purl.obolibrary.org/obo/GAZ_00030981"/>
        <obo:IAO_0000115>A district of Port Said.</obo:IAO_0000115>
        <oboInOwl:hasOBONamespace>GAZ</oboInOwl:hasOBONamespace>
        <oboInOwl:id>GAZ:00030984</oboInOwl:id>
        <rdfs:label>Hai Al Janob (South)</rdfs:label>
    </owl:NamedIndividual>
    


    <!-- http://purl.obolibrary.org/obo/GAZ_00030985 -->

    <owl:NamedIndividual rdf:about="http://purl.obolibrary.org/obo/GAZ_00030985">
        <obo:RO_0001025 rdf:resource="http://purl.obolibrary.org/obo/GAZ_00000646"/>
        <obo:IAO_0000115>A populated place. A city in Asyut Governorate.</obo:IAO_0000115>
        <oboInOwl:hasOBONamespace>GAZ</oboInOwl:hasOBONamespace>
        <oboInOwl:id>GAZ:00030985</oboInOwl:id>
        <rdfs:label>el Badari</rdfs:label>
    </owl:NamedIndividual>
    


    <!-- http://purl.obolibrary.org/obo/GAZ_00030986 -->

    <owl:NamedIndividual rdf:about="http://purl.obolibrary.org/obo/GAZ_00030986">
        <rdf:type rdf:resource="http://purl.obolibrary.org/obo/ENVO_00000004"/>
        <obo:RO_0001025 rdf:resource="http://purl.obolibrary.org/obo/GAZ_00030981"/>
        <obo:IAO_0000115>A district of Port Said.</obo:IAO_0000115>
        <oboInOwl:hasOBONamespace>GAZ</oboInOwl:hasOBONamespace>
        <oboInOwl:id>GAZ:00030986</oboInOwl:id>
        <rdfs:label>Port Fouad</rdfs:label>
    </owl:NamedIndividual>
    


    <!-- http://purl.obolibrary.org/obo/GAZ_00030987 -->

    <owl:NamedIndividual rdf:about="http://purl.obolibrary.org/obo/GAZ_00030987">
        <rdf:type rdf:resource="http://purl.obolibrary.org/obo/ENVO_00000004"/>
        <obo:RO_0001025 rdf:resource="http://purl.obolibrary.org/obo/GAZ_00030981"/>
        <obo:IAO_0000115>A district of Port Said.</obo:IAO_0000115>
        <oboInOwl:hasOBONamespace>GAZ</oboInOwl:hasOBONamespace>
        <oboInOwl:id>GAZ:00030987</oboInOwl:id>
        <rdfs:label>Hai El Dawahi</rdfs:label>
    </owl:NamedIndividual>
    


    <!-- http://purl.obolibrary.org/obo/GAZ_00030988 -->

    <owl:NamedIndividual rdf:about="http://purl.obolibrary.org/obo/GAZ_00030988">
        <rdf:type rdf:resource="http://purl.obolibrary.org/obo/ENVO_00000004"/>
        <obo:RO_0001025 rdf:resource="http://purl.obolibrary.org/obo/GAZ_00030981"/>
        <obo:IAO_0000115>A district of Port Said.</obo:IAO_0000115>
        <oboInOwl:hasOBONamespace>GAZ</oboInOwl:hasOBONamespace>
        <oboInOwl:id>GAZ:00030988</oboInOwl:id>
        <rdfs:label>Hai El Manakh</rdfs:label>
    </owl:NamedIndividual>
    


    <!-- http://purl.obolibrary.org/obo/GAZ_00030989 -->

    <owl:NamedIndividual rdf:about="http://purl.obolibrary.org/obo/GAZ_00030989">
        <obo:RO_0001025 rdf:resource="http://purl.obolibrary.org/obo/GAZ_00000646"/>
        <obo:IAO_0000115>A city located near the city of Abnub in the Asyut Governorate.</obo:IAO_0000115>
        <oboInOwl:hasOBONamespace>GAZ</oboInOwl:hasOBONamespace>
        <oboInOwl:id>GAZ:00030989</oboInOwl:id>
        <rdfs:label>el Fateh</rdfs:label>
    </owl:NamedIndividual>
    


    <!-- http://purl.obolibrary.org/obo/GAZ_00030990 -->

    <owl:NamedIndividual rdf:about="http://purl.obolibrary.org/obo/GAZ_00030990">
        <obo:RO_0001025 rdf:resource="http://purl.obolibrary.org/obo/GAZ_00000646"/>
        <obo:IAO_0000115>An administrative region (markaz) of Asyut Governorate.</obo:IAO_0000115>
        <oboInOwl:hasOBONamespace>GAZ</oboInOwl:hasOBONamespace>
        <oboInOwl:id>GAZ:00030990</oboInOwl:id>
        <rdfs:label>Dairut Region</rdfs:label>
    </owl:NamedIndividual>
    


    <!-- http://purl.obolibrary.org/obo/GAZ_00030991 -->

    <owl:NamedIndividual rdf:about="http://purl.obolibrary.org/obo/GAZ_00030991">
        <obo:RO_0001025 rdf:resource="http://purl.obolibrary.org/obo/GAZ_00000646"/>
        <obo:IAO_0000115>A city located near the city of Abutig in the Asyut Governorate.</obo:IAO_0000115>
        <oboInOwl:hasOBONamespace>GAZ</oboInOwl:hasOBONamespace>
        <oboInOwl:id>GAZ:00030991</oboInOwl:id>
        <rdfs:label>el Ghanayem</rdfs:label>
    </owl:NamedIndividual>
    


    <!-- http://purl.obolibrary.org/obo/GAZ_00030992 -->

    <owl:NamedIndividual rdf:about="http://purl.obolibrary.org/obo/GAZ_00030992">
        <obo:RO_0001025 rdf:resource="http://purl.obolibrary.org/obo/GAZ_00000646"/>
        <obo:IAO_0000115>An administrative region (markaz) of Asyut Governorate.</obo:IAO_0000115>
        <oboInOwl:hasOBONamespace>GAZ</oboInOwl:hasOBONamespace>
        <oboInOwl:id>GAZ:00030992</oboInOwl:id>
        <rdfs:label>Abutig Region</rdfs:label>
    </owl:NamedIndividual>
    


    <!-- http://purl.obolibrary.org/obo/GAZ_00030993 -->

    <owl:NamedIndividual rdf:about="http://purl.obolibrary.org/obo/GAZ_00030993">
        <obo:RO_0001025 rdf:resource="http://purl.obolibrary.org/obo/GAZ_00000646"/>
        <obo:IAO_0000115>An administrative region (markaz) of Asyut Governorate.</obo:IAO_0000115>
        <oboInOwl:hasOBONamespace>GAZ</oboInOwl:hasOBONamespace>
        <oboInOwl:id>GAZ:00030993</oboInOwl:id>
        <rdfs:label>Sahel Selim Region</rdfs:label>
    </owl:NamedIndividual>
    


    <!-- http://purl.obolibrary.org/obo/GAZ_00030994 -->

    <owl:NamedIndividual rdf:about="http://purl.obolibrary.org/obo/GAZ_00030994">
        <obo:RO_0001025 rdf:resource="http://purl.obolibrary.org/obo/GAZ_00000646"/>
        <obo:IAO_0000115>An administrative region (markaz) of Asyut Governorate.</obo:IAO_0000115>
        <oboInOwl:hasOBONamespace>GAZ</oboInOwl:hasOBONamespace>
        <oboInOwl:id>GAZ:00030994</oboInOwl:id>
        <rdfs:label>Abnub Region</rdfs:label>
    </owl:NamedIndividual>
    


    <!-- http://purl.obolibrary.org/obo/GAZ_00030995 -->

    <owl:NamedIndividual rdf:about="http://purl.obolibrary.org/obo/GAZ_00030995">
        <obo:RO_0001025 rdf:resource="http://purl.obolibrary.org/obo/GAZ_00000646"/>
        <obo:IAO_0000115>An administrative region (markaz) of Asyut Governorate.</obo:IAO_0000115>
        <oboInOwl:hasOBONamespace>GAZ</oboInOwl:hasOBONamespace>
        <oboInOwl:id>GAZ:00030995</oboInOwl:id>
        <rdfs:label>Sedfa Region</rdfs:label>
    </owl:NamedIndividual>
    


    <!-- http://purl.obolibrary.org/obo/GAZ_00030996 -->

    <owl:NamedIndividual rdf:about="http://purl.obolibrary.org/obo/GAZ_00030996">
        <obo:RO_0001025 rdf:resource="http://purl.obolibrary.org/obo/GAZ_00000646"/>
        <obo:IAO_0000115>An administrative region (markaz) of Asyut Governorate.</obo:IAO_0000115>
        <oboInOwl:hasOBONamespace>GAZ</oboInOwl:hasOBONamespace>
        <oboInOwl:id>GAZ:00030996</oboInOwl:id>
        <rdfs:label>Asyut Region</rdfs:label>
    </owl:NamedIndividual>
    


    <!-- http://purl.obolibrary.org/obo/GAZ_00030997 -->

    <owl:NamedIndividual rdf:about="http://purl.obolibrary.org/obo/GAZ_00030997">
        <obo:RO_0001025 rdf:resource="http://purl.obolibrary.org/obo/GAZ_00000646"/>
        <obo:IAO_0000115>An administrative region (markaz) of Asyut Governorate.</obo:IAO_0000115>
        <oboInOwl:hasOBONamespace>GAZ</oboInOwl:hasOBONamespace>
        <oboInOwl:id>GAZ:00030997</oboInOwl:id>
        <rdfs:label>Manfalut Region</rdfs:label>
    </owl:NamedIndividual>
    


    <!-- http://purl.obolibrary.org/obo/GAZ_00030998 -->

    <owl:NamedIndividual rdf:about="http://purl.obolibrary.org/obo/GAZ_00030998">
        <obo:RO_0001025 rdf:resource="http://purl.obolibrary.org/obo/GAZ_00000646"/>
        <obo:IAO_0000115>A city located on the west bank of the Nile, in the Asyut Governorate.</obo:IAO_0000115>
        <oboInOwl:hasOBONamespace>GAZ</oboInOwl:hasOBONamespace>
        <oboInOwl:id>GAZ:00030998</oboInOwl:id>
        <rdfs:label>el-Qusiya</rdfs:label>
    </owl:NamedIndividual>
    


    <!-- http://purl.obolibrary.org/obo/GAZ_00030999 -->

    <owl:NamedIndividual rdf:about="http://purl.obolibrary.org/obo/GAZ_00030999">
        <obo:RO_0001025 rdf:resource="http://purl.obolibrary.org/obo/GAZ_00000662"/>
        <obo:IAO_0000115>An administrative region (markaz) of Sharqia Governorate.</obo:IAO_0000115>
        <oboInOwl:hasOBONamespace>GAZ</oboInOwl:hasOBONamespace>
        <oboInOwl:id>GAZ:00030999</oboInOwl:id>
        <rdfs:label>Menya Al Qamh Region</rdfs:label>
    </owl:NamedIndividual>
    


    <!-- http://purl.obolibrary.org/obo/GAZ_00031000 -->

    <owl:NamedIndividual rdf:about="http://purl.obolibrary.org/obo/GAZ_00031000">
        <obo:RO_0001025 rdf:resource="http://purl.obolibrary.org/obo/GAZ_00000662"/>
        <obo:IAO_0000115>An administrative region (markaz) of Sharqia Governorate.</obo:IAO_0000115>
        <oboInOwl:hasOBONamespace>GAZ</oboInOwl:hasOBONamespace>
        <oboInOwl:id>GAZ:00031000</oboInOwl:id>
        <rdfs:label>Faqous Region</rdfs:label>
    </owl:NamedIndividual>
    


    <!-- http://purl.obolibrary.org/obo/GAZ_00031001 -->

    <owl:NamedIndividual rdf:about="http://purl.obolibrary.org/obo/GAZ_00031001">
        <obo:RO_0001025 rdf:resource="http://purl.obolibrary.org/obo/GAZ_00000662"/>
        <obo:IAO_0000115>An administrative region (markaz) of Sharqia Governorate.</obo:IAO_0000115>
        <oboInOwl:hasOBONamespace>GAZ</oboInOwl:hasOBONamespace>
        <oboInOwl:id>GAZ:00031001</oboInOwl:id>
        <rdfs:label>Belbeis Region</rdfs:label>
    </owl:NamedIndividual>
    


    <!-- http://purl.obolibrary.org/obo/GAZ_00031002 -->

    <owl:NamedIndividual rdf:about="http://purl.obolibrary.org/obo/GAZ_00031002">
        <obo:RO_0001025 rdf:resource="http://purl.obolibrary.org/obo/GAZ_00000662"/>
        <obo:IAO_0000115>An administrative region (markaz) of Sharqia Governorate.</obo:IAO_0000115>
        <oboInOwl:hasOBONamespace>GAZ</oboInOwl:hasOBONamespace>
        <oboInOwl:id>GAZ:00031002</oboInOwl:id>
        <rdfs:label>Zaqaziq Region</rdfs:label>
    </owl:NamedIndividual>
    


    <!-- http://purl.obolibrary.org/obo/GAZ_00031003 -->

    <owl:NamedIndividual rdf:about="http://purl.obolibrary.org/obo/GAZ_00031003">
        <obo:RO_0001025 rdf:resource="http://purl.obolibrary.org/obo/GAZ_00000662"/>
        <obo:IAO_0000115>An administrative region (markaz) of Sharqia Governorate.</obo:IAO_0000115>
        <oboInOwl:hasOBONamespace>GAZ</oboInOwl:hasOBONamespace>
        <oboInOwl:id>GAZ:00031003</oboInOwl:id>
        <rdfs:label>Abu Kabeer Region</rdfs:label>
    </owl:NamedIndividual>
    


    <!-- http://purl.obolibrary.org/obo/GAZ_00031004 -->

    <owl:NamedIndividual rdf:about="http://purl.obolibrary.org/obo/GAZ_00031004">
        <obo:RO_0001025 rdf:resource="http://purl.obolibrary.org/obo/GAZ_00000662"/>
        <obo:IAO_0000115>An administrative region (markaz) of Sharqia Governorate.</obo:IAO_0000115>
        <oboInOwl:hasOBONamespace>GAZ</oboInOwl:hasOBONamespace>
        <oboInOwl:id>GAZ:00031004</oboInOwl:id>
        <rdfs:label>Kafr Saqr Region</rdfs:label>
    </owl:NamedIndividual>
    


    <!-- http://purl.obolibrary.org/obo/GAZ_00031005 -->

    <owl:NamedIndividual rdf:about="http://purl.obolibrary.org/obo/GAZ_00031005">
        <obo:RO_0001025 rdf:resource="http://purl.obolibrary.org/obo/GAZ_00000662"/>
        <obo:IAO_0000115>An administrative region (kism) of Sharqia Governorate.</obo:IAO_0000115>
        <oboInOwl:hasOBONamespace>GAZ</oboInOwl:hasOBONamespace>
        <oboInOwl:id>GAZ:00031005</oboInOwl:id>
        <rdfs:label>Kism Al Qanayat</rdfs:label>
    </owl:NamedIndividual>
    


    <!-- http://purl.obolibrary.org/obo/GAZ_00031006 -->

    <owl:NamedIndividual rdf:about="http://purl.obolibrary.org/obo/GAZ_00031006">
        <obo:RO_0001025 rdf:resource="http://purl.obolibrary.org/obo/GAZ_00000662"/>
        <obo:IAO_0000115>An administrative region (markaz) of Sharqia Governorate.</obo:IAO_0000115>
        <oboInOwl:hasOBONamespace>GAZ</oboInOwl:hasOBONamespace>
        <oboInOwl:id>GAZ:00031006</oboInOwl:id>
        <rdfs:label>Deyarb Najm Region</rdfs:label>
    </owl:NamedIndividual>
    


    <!-- http://purl.obolibrary.org/obo/GAZ_00031007 -->

    <owl:NamedIndividual rdf:about="http://purl.obolibrary.org/obo/GAZ_00031007">
        <obo:RO_0001025 rdf:resource="http://purl.obolibrary.org/obo/GAZ_00000662"/>
        <obo:IAO_0000115>An administrative region (markaz) of Sharqia Governorate.</obo:IAO_0000115>
        <oboInOwl:hasOBONamespace>GAZ</oboInOwl:hasOBONamespace>
        <oboInOwl:id>GAZ:00031007</oboInOwl:id>
        <rdfs:label>Hehya Region</rdfs:label>
    </owl:NamedIndividual>
    


    <!-- http://purl.obolibrary.org/obo/GAZ_00031008 -->

    <owl:NamedIndividual rdf:about="http://purl.obolibrary.org/obo/GAZ_00031008">
        <obo:RO_0001025 rdf:resource="http://purl.obolibrary.org/obo/GAZ_00000662"/>
        <obo:IAO_0000115>An administrative region (markaz) of Sharqia Governorate.</obo:IAO_0000115>
        <oboInOwl:hasOBONamespace>GAZ</oboInOwl:hasOBONamespace>
        <oboInOwl:id>GAZ:00031008</oboInOwl:id>
        <rdfs:label>Abou Hammaad Region</rdfs:label>
    </owl:NamedIndividual>
    


    <!-- http://purl.obolibrary.org/obo/GAZ_00031009 -->

    <owl:NamedIndividual rdf:about="http://purl.obolibrary.org/obo/GAZ_00031009">
        <obo:RO_0001025 rdf:resource="http://purl.obolibrary.org/obo/GAZ_00000662"/>
        <obo:IAO_0000115>An administrative region (markaz) of Sharqia Governorate.</obo:IAO_0000115>
        <oboInOwl:hasOBONamespace>GAZ</oboInOwl:hasOBONamespace>
        <oboInOwl:id>GAZ:00031009</oboInOwl:id>
        <rdfs:label>Al Husaineya Region</rdfs:label>
    </owl:NamedIndividual>
    


    <!-- http://purl.obolibrary.org/obo/GAZ_00031010 -->

    <owl:NamedIndividual rdf:about="http://purl.obolibrary.org/obo/GAZ_00031010">
        <obo:RO_0001025 rdf:resource="http://purl.obolibrary.org/obo/GAZ_00000662"/>
        <obo:IAO_0000115>An administrative region (markaz) of Sharqia Governorate.</obo:IAO_0000115>
        <oboInOwl:hasOBONamespace>GAZ</oboInOwl:hasOBONamespace>
        <oboInOwl:id>GAZ:00031010</oboInOwl:id>
        <rdfs:label>Al Ebrahemeyah Region</rdfs:label>
    </owl:NamedIndividual>
    


    <!-- http://purl.obolibrary.org/obo/GAZ_00031011 -->

    <owl:NamedIndividual rdf:about="http://purl.obolibrary.org/obo/GAZ_00031011">
        <obo:RO_0001025 rdf:resource="http://purl.obolibrary.org/obo/GAZ_00000662"/>
        <obo:IAO_0000115>An administrative region (markaz) of Sharqia Governorate.</obo:IAO_0000115>
        <oboInOwl:hasOBONamespace>GAZ</oboInOwl:hasOBONamespace>
        <oboInOwl:id>GAZ:00031011</oboInOwl:id>
        <rdfs:label>Awlaad Saqr Region</rdfs:label>
    </owl:NamedIndividual>
    


    <!-- http://purl.obolibrary.org/obo/GAZ_00031012 -->

    <owl:NamedIndividual rdf:about="http://purl.obolibrary.org/obo/GAZ_00031012">
        <obo:RO_0001025 rdf:resource="http://purl.obolibrary.org/obo/GAZ_00051197"/>
        <obo:RO_0001025 rdf:resource="http://purl.obolibrary.org/obo/GAZ_00066407"/>
        <obo:IAO_0000115>One of the seven oases of the Western Desert of Egypt (part of the Libyan Desert). Dakhla Oasis is located at 350 km from the Nile Valley and is also situated between the oases of Farafra and Kharga. It measures some 80 km from east to west and about 25 km from north to south.</obo:IAO_0000115>
        <oboInOwl:hasOBONamespace>GAZ</oboInOwl:hasOBONamespace>
        <oboInOwl:id>GAZ:00031012</oboInOwl:id>
        <rdfs:label>Dakhla Oasis</rdfs:label>
    </owl:NamedIndividual>
    


    <!-- http://purl.obolibrary.org/obo/GAZ_00031013 -->

    <owl:NamedIndividual rdf:about="http://purl.obolibrary.org/obo/GAZ_00031013">
        <obo:RO_0001025 rdf:resource="http://purl.obolibrary.org/obo/GAZ_00051197"/>
        <obo:RO_0001025 rdf:resource="http://purl.obolibrary.org/obo/GAZ_00066408"/>
        <obo:IAO_0000115>The southernmost of Egypt&apos;s five western oases. It is located in the Libyan Desert, about 200 km to the west of the Nile valley, and is some 150 km long. It is located in and is the capital of El Wadi el Gedid governorate.</obo:IAO_0000115>
        <oboInOwl:hasOBONamespace>GAZ</oboInOwl:hasOBONamespace>
        <oboInOwl:id>GAZ:00031013</oboInOwl:id>
        <rdfs:label>Kharga Oasis</rdfs:label>
    </owl:NamedIndividual>
    


    <!-- http://purl.obolibrary.org/obo/GAZ_00031014 -->

    <owl:NamedIndividual rdf:about="http://purl.obolibrary.org/obo/GAZ_00031014">
        <obo:RO_0001025 rdf:resource="http://purl.obolibrary.org/obo/GAZ_00051197"/>
        <obo:RO_0001025 rdf:resource="http://purl.obolibrary.org/obo/GAZ_00241998"/>
        <oboInOwl:hasOBONamespace>GAZ</oboInOwl:hasOBONamespace>
        <oboInOwl:id>GAZ:00031014</oboInOwl:id>
        <rdfs:label>Baris Oasis</rdfs:label>
    </owl:NamedIndividual>
    


    <!-- http://purl.obolibrary.org/obo/GAZ_00031015 -->

    <owl:NamedIndividual rdf:about="http://purl.obolibrary.org/obo/GAZ_00031015">
        <obo:RO_0001025 rdf:resource="http://purl.obolibrary.org/obo/GAZ_00051197"/>
        <obo:RO_0001025 rdf:resource="http://purl.obolibrary.org/obo/GAZ_00066406"/>
        <obo:IAO_0000115>The smallest oasis located in Western Egypt. It is located in the Libyan Desert, approximately mid-way between Dakhla and Bahariya.</obo:IAO_0000115>
        <oboInOwl:hasOBONamespace>GAZ</oboInOwl:hasOBONamespace>
        <oboInOwl:id>GAZ:00031015</oboInOwl:id>
        <rdfs:label>Farafra Oasis</rdfs:label>
    </owl:NamedIndividual>
    


    <!-- http://purl.obolibrary.org/obo/GAZ_00031016 -->

    <owl:NamedIndividual rdf:about="http://purl.obolibrary.org/obo/GAZ_00031016">
        <obo:RO_0001025 rdf:resource="http://purl.obolibrary.org/obo/GAZ_00000661"/>
        <obo:IAO_0000115>An administrative region (markaz) of Qalyubia Governorate.</obo:IAO_0000115>
        <oboInOwl:hasOBONamespace>GAZ</oboInOwl:hasOBONamespace>
        <oboInOwl:id>GAZ:00031016</oboInOwl:id>
        <rdfs:label>Banha Region</rdfs:label>
    </owl:NamedIndividual>
    


    <!-- http://purl.obolibrary.org/obo/GAZ_00031017 -->

    <owl:NamedIndividual rdf:about="http://purl.obolibrary.org/obo/GAZ_00031017">
        <obo:RO_0001025 rdf:resource="http://purl.obolibrary.org/obo/GAZ_00000661"/>
        <obo:IAO_0000115>A populated place.</obo:IAO_0000115>
        <oboInOwl:hasOBONamespace>GAZ</oboInOwl:hasOBONamespace>
        <oboInOwl:id>GAZ:00031017</oboInOwl:id>
        <rdfs:label>Abu Zaabal</rdfs:label>
    </owl:NamedIndividual>
    


    <!-- http://purl.obolibrary.org/obo/GAZ_00031018 -->

    <owl:NamedIndividual rdf:about="http://purl.obolibrary.org/obo/GAZ_00031018">
        <obo:RO_0001025 rdf:resource="http://purl.obolibrary.org/obo/GAZ_00000661"/>
        <obo:IAO_0000115>An administrative region (markaz) of Qalyubia Governorate.</obo:IAO_0000115>
        <oboInOwl:hasOBONamespace>GAZ</oboInOwl:hasOBONamespace>
        <oboInOwl:id>GAZ:00031018</oboInOwl:id>
        <rdfs:label>Khanka Region</rdfs:label>
    </owl:NamedIndividual>
    


    <!-- http://purl.obolibrary.org/obo/GAZ_00031019 -->

    <owl:NamedIndividual rdf:about="http://purl.obolibrary.org/obo/GAZ_00031019">
        <obo:RO_0001025 rdf:resource="http://purl.obolibrary.org/obo/GAZ_00000661"/>
        <obo:IAO_0000115>An administrative region (kism) of Qalyubia Governorate.</obo:IAO_0000115>
        <oboInOwl:hasOBONamespace>GAZ</oboInOwl:hasOBONamespace>
        <oboInOwl:id>GAZ:00031019</oboInOwl:id>
        <rdfs:label>Kism Qaha</rdfs:label>
    </owl:NamedIndividual>
    


    <!-- http://purl.obolibrary.org/obo/GAZ_00031020 -->

    <owl:NamedIndividual rdf:about="http://purl.obolibrary.org/obo/GAZ_00031020">
        <obo:RO_0001025 rdf:resource="http://purl.obolibrary.org/obo/GAZ_00000661"/>
        <obo:IAO_0000115>An administrative region (markaz) of Qalyubia Governorate.</obo:IAO_0000115>
        <oboInOwl:hasOBONamespace>GAZ</oboInOwl:hasOBONamespace>
        <oboInOwl:id>GAZ:00031020</oboInOwl:id>
        <rdfs:label>Qalyub Region</rdfs:label>
    </owl:NamedIndividual>
    


    <!-- http://purl.obolibrary.org/obo/GAZ_00031021 -->

    <owl:NamedIndividual rdf:about="http://purl.obolibrary.org/obo/GAZ_00031021">
        <obo:RO_0001025 rdf:resource="http://purl.obolibrary.org/obo/GAZ_00000661"/>
        <obo:IAO_0000115>An administrative region (markaz) of Qalyubia Governorate.</obo:IAO_0000115>
        <oboInOwl:hasOBONamespace>GAZ</oboInOwl:hasOBONamespace>
        <oboInOwl:id>GAZ:00031021</oboInOwl:id>
        <rdfs:label>Tukh Region</rdfs:label>
    </owl:NamedIndividual>
    


    <!-- http://purl.obolibrary.org/obo/GAZ_00031022 -->

    <owl:NamedIndividual rdf:about="http://purl.obolibrary.org/obo/GAZ_00031022">
        <obo:RO_0001025 rdf:resource="http://purl.obolibrary.org/obo/GAZ_00000661"/>
        <oboInOwl:hasOBONamespace>GAZ</oboInOwl:hasOBONamespace>
        <oboInOwl:id>GAZ:00031022</oboInOwl:id>
        <rdfs:label>Shubra-el-Khema Region</rdfs:label>
    </owl:NamedIndividual>
    


    <!-- http://purl.obolibrary.org/obo/GAZ_00031023 -->

    <owl:NamedIndividual rdf:about="http://purl.obolibrary.org/obo/GAZ_00031023">
        <obo:RO_0001025 rdf:resource="http://purl.obolibrary.org/obo/GAZ_00000661"/>
        <obo:IAO_0000115>An administrative region (markaz) of Qalyubia Governorate.</obo:IAO_0000115>
        <oboInOwl:hasOBONamespace>GAZ</oboInOwl:hasOBONamespace>
        <oboInOwl:id>GAZ:00031023</oboInOwl:id>
        <rdfs:label>Shibin Al-Qanater Region</rdfs:label>
    </owl:NamedIndividual>
    


    <!-- http://purl.obolibrary.org/obo/GAZ_00031024 -->

    <owl:NamedIndividual rdf:about="http://purl.obolibrary.org/obo/GAZ_00031024">
        <obo:RO_0001025 rdf:resource="http://purl.obolibrary.org/obo/GAZ_00000650"/>
        <obo:IAO_0000115>An administrative region (markaz) of Minya Governorate.</obo:IAO_0000115>
        <oboInOwl:hasOBONamespace>GAZ</oboInOwl:hasOBONamespace>
        <oboInOwl:id>GAZ:00031024</oboInOwl:id>
        <rdfs:label>Maghagha Region</rdfs:label>
    </owl:NamedIndividual>
    


    <!-- http://purl.obolibrary.org/obo/GAZ_00031025 -->

    <owl:NamedIndividual rdf:about="http://purl.obolibrary.org/obo/GAZ_00031025">
        <obo:RO_0001025 rdf:resource="http://purl.obolibrary.org/obo/GAZ_00000650"/>
        <obo:IAO_0000115>An administrative region (markaz) of Minya Governorate.</obo:IAO_0000115>
        <oboInOwl:hasOBONamespace>GAZ</oboInOwl:hasOBONamespace>
        <oboInOwl:id>GAZ:00031025</oboInOwl:id>
        <rdfs:label>Samalut Region</rdfs:label>
    </owl:NamedIndividual>
    


    <!-- http://purl.obolibrary.org/obo/GAZ_00031026 -->

    <owl:NamedIndividual rdf:about="http://purl.obolibrary.org/obo/GAZ_00031026">
        <obo:RO_0001025 rdf:resource="http://purl.obolibrary.org/obo/GAZ_00000650"/>
        <obo:IAO_0000115>An administrative region (markaz) of Minya Governorate.</obo:IAO_0000115>
        <oboInOwl:hasOBONamespace>GAZ</oboInOwl:hasOBONamespace>
        <oboInOwl:id>GAZ:00031026</oboInOwl:id>
        <rdfs:label>Beni Mazar Region</rdfs:label>
    </owl:NamedIndividual>
    


    <!-- http://purl.obolibrary.org/obo/GAZ_00031027 -->

    <owl:NamedIndividual rdf:about="http://purl.obolibrary.org/obo/GAZ_00031027">
        <obo:RO_0001025 rdf:resource="http://purl.obolibrary.org/obo/GAZ_00000650"/>
        <obo:IAO_0000115>An administrative region (markaz) of Minya Governorate.</obo:IAO_0000115>
        <oboInOwl:hasOBONamespace>GAZ</oboInOwl:hasOBONamespace>
        <oboInOwl:id>GAZ:00031027</oboInOwl:id>
        <rdfs:label>Minya Region</rdfs:label>
    </owl:NamedIndividual>
    


    <!-- http://purl.obolibrary.org/obo/GAZ_00031028 -->

    <owl:NamedIndividual rdf:about="http://purl.obolibrary.org/obo/GAZ_00031028">
        <obo:RO_0001025 rdf:resource="http://purl.obolibrary.org/obo/GAZ_00000650"/>
        <obo:IAO_0000115>An administrative region (markaz) of Minya Governorate.</obo:IAO_0000115>
        <oboInOwl:hasOBONamespace>GAZ</oboInOwl:hasOBONamespace>
        <oboInOwl:id>GAZ:00031028</oboInOwl:id>
        <rdfs:label>Mallawi Region</rdfs:label>
    </owl:NamedIndividual>
    


    <!-- http://purl.obolibrary.org/obo/GAZ_00031029 -->

    <owl:NamedIndividual rdf:about="http://purl.obolibrary.org/obo/GAZ_00031029">
        <obo:RO_0001025 rdf:resource="http://purl.obolibrary.org/obo/GAZ_00000650"/>
        <obo:IAO_0000115>An administrative region (markaz) of Minya Governorate.</obo:IAO_0000115>
        <oboInOwl:hasOBONamespace>GAZ</oboInOwl:hasOBONamespace>
        <oboInOwl:id>GAZ:00031029</oboInOwl:id>
        <rdfs:label>Abu Qirqas Region</rdfs:label>
    </owl:NamedIndividual>
    


    <!-- http://purl.obolibrary.org/obo/GAZ_00031030 -->

    <owl:NamedIndividual rdf:about="http://purl.obolibrary.org/obo/GAZ_00031030">
        <obo:RO_0001025 rdf:resource="http://purl.obolibrary.org/obo/GAZ_00000650"/>
        <obo:IAO_0000115>An administrative region (markaz) of Minya Governorate.</obo:IAO_0000115>
        <oboInOwl:hasOBONamespace>GAZ</oboInOwl:hasOBONamespace>
        <oboInOwl:id>GAZ:00031030</oboInOwl:id>
        <rdfs:label>Deir Mawas Region</rdfs:label>
    </owl:NamedIndividual>
    


    <!-- http://purl.obolibrary.org/obo/GAZ_00031031 -->

    <owl:NamedIndividual rdf:about="http://purl.obolibrary.org/obo/GAZ_00031031">
        <obo:RO_0001025 rdf:resource="http://purl.obolibrary.org/obo/GAZ_00000650"/>
        <obo:IAO_0000115>An administrative region (markaz) of Minya Governorate.</obo:IAO_0000115>
        <oboInOwl:hasOBONamespace>GAZ</oboInOwl:hasOBONamespace>
        <oboInOwl:id>GAZ:00031031</oboInOwl:id>
        <rdfs:label>El Idwa Region</rdfs:label>
    </owl:NamedIndividual>
    


    <!-- http://purl.obolibrary.org/obo/GAZ_00031032 -->

    <owl:NamedIndividual rdf:about="http://purl.obolibrary.org/obo/GAZ_00031032">
        <obo:RO_0001025 rdf:resource="http://purl.obolibrary.org/obo/GAZ_00000650"/>
        <obo:IAO_0000115>An administrative region (markaz) of Minya Governorate.</obo:IAO_0000115>
        <oboInOwl:hasOBONamespace>GAZ</oboInOwl:hasOBONamespace>
        <oboInOwl:id>GAZ:00031032</oboInOwl:id>
        <rdfs:label>Matai Region</rdfs:label>
    </owl:NamedIndividual>
    


    <!-- http://purl.obolibrary.org/obo/GAZ_00031033 -->

    <owl:NamedIndividual rdf:about="http://purl.obolibrary.org/obo/GAZ_00031033">
        <obo:RO_0001025 rdf:resource="http://purl.obolibrary.org/obo/GAZ_00000655"/>
        <obo:IAO_0000115>An administrative region (markuz) of Beheira Governorate.</obo:IAO_0000115>
        <oboInOwl:hasOBONamespace>GAZ</oboInOwl:hasOBONamespace>
        <oboInOwl:id>GAZ:00031033</oboInOwl:id>
        <rdfs:label>Damanhur Region</rdfs:label>
    </owl:NamedIndividual>
    


    <!-- http://purl.obolibrary.org/obo/GAZ_00031034 -->

    <owl:NamedIndividual rdf:about="http://purl.obolibrary.org/obo/GAZ_00031034">
        <obo:RO_0001025 rdf:resource="http://purl.obolibrary.org/obo/GAZ_00000655"/>
        <obo:IAO_0000115>An administrative region (markuz) of Beheira Governorate.</obo:IAO_0000115>
        <oboInOwl:hasOBONamespace>GAZ</oboInOwl:hasOBONamespace>
        <oboInOwl:id>GAZ:00031034</oboInOwl:id>
        <rdfs:label>Rosetta Region</rdfs:label>
    </owl:NamedIndividual>
    


    <!-- http://purl.obolibrary.org/obo/GAZ_00039902 -->

    <owl:NamedIndividual rdf:about="http://purl.obolibrary.org/obo/GAZ_00039902">
        <obo:RO_0001025 rdf:resource="http://purl.obolibrary.org/obo/GAZ_00102118"/>
        <obo:IAO_0000115>A group of small islands off of the eastern coast of the Horn of Africa, in the Dact-el-Mayun section of the Bab-el-Mandeb strait.</obo:IAO_0000115>
        <oboInOwl:hasOBONamespace>GAZ</oboInOwl:hasOBONamespace>
        <oboInOwl:id>GAZ:00039902</oboInOwl:id>
        <rdfs:label>Sept Freres</rdfs:label>
    </owl:NamedIndividual>
    


    <!-- http://purl.obolibrary.org/obo/GAZ_00039909 -->

    <owl:NamedIndividual rdf:about="http://purl.obolibrary.org/obo/GAZ_00039909">
        <obo:RO_0001025 rdf:resource="http://purl.obolibrary.org/obo/GAZ_00009683"/>
        <obo:IAO_0000115>An island of the Dahlak Archipelago.</obo:IAO_0000115>
        <oboInOwl:hasOBONamespace>GAZ</oboInOwl:hasOBONamespace>
        <oboInOwl:id>GAZ:00039909</oboInOwl:id>
        <rdfs:label>Harmil Island</rdfs:label>
    </owl:NamedIndividual>
    


    <!-- http://purl.obolibrary.org/obo/GAZ_00039910 -->

    <owl:NamedIndividual rdf:about="http://purl.obolibrary.org/obo/GAZ_00039910">
        <obo:RO_0001025 rdf:resource="http://purl.obolibrary.org/obo/GAZ_00009683"/>
        <obo:IAO_0000115>An island of the Dahlak Archipelago.</obo:IAO_0000115>
        <oboInOwl:hasOBONamespace>GAZ</oboInOwl:hasOBONamespace>
        <oboInOwl:id>GAZ:00039910</oboInOwl:id>
        <rdfs:label>Nora Island</rdfs:label>
    </owl:NamedIndividual>
    


    <!-- http://purl.obolibrary.org/obo/GAZ_00039911 -->

    <owl:NamedIndividual rdf:about="http://purl.obolibrary.org/obo/GAZ_00039911">
        <obo:RO_0001025 rdf:resource="http://purl.obolibrary.org/obo/GAZ_00009683"/>
        <obo:IAO_0000115>An island of the Dahlak Archipelago.</obo:IAO_0000115>
        <oboInOwl:hasOBONamespace>GAZ</oboInOwl:hasOBONamespace>
        <oboInOwl:id>GAZ:00039911</oboInOwl:id>
        <rdfs:label>Dahlak Kebir</rdfs:label>
    </owl:NamedIndividual>
    


    <!-- http://purl.obolibrary.org/obo/GAZ_00039912 -->

    <owl:NamedIndividual rdf:about="http://purl.obolibrary.org/obo/GAZ_00039912">
        <obo:RO_0001025 rdf:resource="http://purl.obolibrary.org/obo/GAZ_00009683"/>
        <obo:IAO_0000115>An island of the Dahlak Archipelago.</obo:IAO_0000115>
        <oboInOwl:hasOBONamespace>GAZ</oboInOwl:hasOBONamespace>
        <oboInOwl:id>GAZ:00039912</oboInOwl:id>
        <rdfs:label>Nahaleg Island</rdfs:label>
    </owl:NamedIndividual>
    


    <!-- http://purl.obolibrary.org/obo/GAZ_00039913 -->

    <owl:NamedIndividual rdf:about="http://purl.obolibrary.org/obo/GAZ_00039913">
        <obo:RO_0001025 rdf:resource="http://purl.obolibrary.org/obo/GAZ_00002456"/>
        <obo:IAO_0000115>An island.</obo:IAO_0000115>
        <oboInOwl:hasOBONamespace>GAZ</oboInOwl:hasOBONamespace>
        <oboInOwl:id>GAZ:00039913</oboInOwl:id>
        <rdfs:label>Massawa Island</rdfs:label>
    </owl:NamedIndividual>
    


    <!-- http://purl.obolibrary.org/obo/GAZ_00039915 -->

    <owl:NamedIndividual rdf:about="http://purl.obolibrary.org/obo/GAZ_00039915">
        <obo:RO_0001025 rdf:resource="http://purl.obolibrary.org/obo/GAZ_00248117"/>
        <obo:IAO_0000115>An island.</obo:IAO_0000115>
        <oboInOwl:hasOBONamespace>GAZ</oboInOwl:hasOBONamespace>
        <oboInOwl:id>GAZ:00039915</oboInOwl:id>
        <rdfs:label>Halba Deset</rdfs:label>
    </owl:NamedIndividual>
    


    <!-- http://purl.obolibrary.org/obo/GAZ_00039916 -->

    <owl:NamedIndividual rdf:about="http://purl.obolibrary.org/obo/GAZ_00039916">
        <obo:RO_0001025 rdf:resource="http://purl.obolibrary.org/obo/GAZ_00002456"/>
        <obo:IAO_0000115>Islands.</obo:IAO_0000115>
        <oboInOwl:hasOBONamespace>GAZ</oboInOwl:hasOBONamespace>
        <oboInOwl:id>GAZ:00039916</oboInOwl:id>
        <rdfs:label>Howakil Islands</rdfs:label>
    </owl:NamedIndividual>
    


    <!-- http://purl.obolibrary.org/obo/GAZ_00039917 -->

    <owl:NamedIndividual rdf:about="http://purl.obolibrary.org/obo/GAZ_00039917">
        <obo:RO_0001025 rdf:resource="http://purl.obolibrary.org/obo/GAZ_00009683"/>
        <obo:IAO_0000115>An island of the Dahlak Archipelago.</obo:IAO_0000115>
        <oboInOwl:hasOBONamespace>GAZ</oboInOwl:hasOBONamespace>
        <oboInOwl:id>GAZ:00039917</oboInOwl:id>
        <rdfs:label>Isra-Tu Island</rdfs:label>
    </owl:NamedIndividual>
    


    <!-- http://purl.obolibrary.org/obo/GAZ_00039918 -->

    <owl:NamedIndividual rdf:about="http://purl.obolibrary.org/obo/GAZ_00039918">
        <obo:RO_0001025 rdf:resource="http://purl.obolibrary.org/obo/GAZ_00009683"/>
        <obo:IAO_0000115>An island of the Dahlak Archipelago.</obo:IAO_0000115>
        <oboInOwl:hasOBONamespace>GAZ</oboInOwl:hasOBONamespace>
        <oboInOwl:id>GAZ:00039918</oboInOwl:id>
        <rdfs:label>Shumma Island</rdfs:label>
    </owl:NamedIndividual>
    


    <!-- http://purl.obolibrary.org/obo/GAZ_00039919 -->

    <owl:NamedIndividual rdf:about="http://purl.obolibrary.org/obo/GAZ_00039919">
        <obo:RO_0001025 rdf:resource="http://purl.obolibrary.org/obo/GAZ_00009683"/>
        <obo:IAO_0000115>An island of the Dahlak Archipelago.</obo:IAO_0000115>
        <oboInOwl:hasOBONamespace>GAZ</oboInOwl:hasOBONamespace>
        <oboInOwl:id>GAZ:00039919</oboInOwl:id>
        <rdfs:label>Harat Island</rdfs:label>
    </owl:NamedIndividual>
    


    <!-- http://purl.obolibrary.org/obo/GAZ_00039920 -->

    <owl:NamedIndividual rdf:about="http://purl.obolibrary.org/obo/GAZ_00039920">
        <obo:RO_0001025 rdf:resource="http://purl.obolibrary.org/obo/GAZ_00009683"/>
        <obo:IAO_0000115>An island of the Dahlak Archipelago.</obo:IAO_0000115>
        <oboInOwl:hasOBONamespace>GAZ</oboInOwl:hasOBONamespace>
        <oboInOwl:id>GAZ:00039920</oboInOwl:id>
        <rdfs:label>Dissei Island</rdfs:label>
    </owl:NamedIndividual>
    


    <!-- http://purl.obolibrary.org/obo/GAZ_00039921 -->

    <owl:NamedIndividual rdf:about="http://purl.obolibrary.org/obo/GAZ_00039921">
        <obo:RO_0001025 rdf:resource="http://purl.obolibrary.org/obo/GAZ_00009683"/>
        <obo:IAO_0000115>An island of the Dahlak Archipelago.</obo:IAO_0000115>
        <oboInOwl:hasOBONamespace>GAZ</oboInOwl:hasOBONamespace>
        <oboInOwl:id>GAZ:00039921</oboInOwl:id>
        <rdfs:label>Erwa Island</rdfs:label>
    </owl:NamedIndividual>
    


    <!-- http://purl.obolibrary.org/obo/GAZ_00039922 -->

    <owl:NamedIndividual rdf:about="http://purl.obolibrary.org/obo/GAZ_00039922">
        <obo:RO_0001025 rdf:resource="http://purl.obolibrary.org/obo/GAZ_00009683"/>
        <obo:IAO_0000115>An island of the Dahlak Archipelago.</obo:IAO_0000115>
        <oboInOwl:hasOBONamespace>GAZ</oboInOwl:hasOBONamespace>
        <oboInOwl:id>GAZ:00039922</oboInOwl:id>
        <rdfs:label>Dohul Island</rdfs:label>
    </owl:NamedIndividual>
    


    <!-- http://purl.obolibrary.org/obo/GAZ_00039923 -->

    <owl:NamedIndividual rdf:about="http://purl.obolibrary.org/obo/GAZ_00039923">
        <obo:RO_0001025 rdf:resource="http://purl.obolibrary.org/obo/GAZ_00009683"/>
        <obo:IAO_0000115>An island of the Dahlak Archipelago.</obo:IAO_0000115>
        <oboInOwl:hasOBONamespace>GAZ</oboInOwl:hasOBONamespace>
        <oboInOwl:id>GAZ:00039923</oboInOwl:id>
        <rdfs:label>Dhuladhiya Island</rdfs:label>
    </owl:NamedIndividual>
    


    <!-- http://purl.obolibrary.org/obo/GAZ_00043227 -->

    <owl:NamedIndividual rdf:about="http://purl.obolibrary.org/obo/GAZ_00043227">
        <obo:IAO_0000115>An island located just to the south of Aswan.</obo:IAO_0000115>
        <oboInOwl:hasOBONamespace>GAZ</oboInOwl:hasOBONamespace>
        <oboInOwl:id>GAZ:00043227</oboInOwl:id>
        <rdfs:label>Sehel Island</rdfs:label>
    </owl:NamedIndividual>
    


    <!-- http://purl.obolibrary.org/obo/GAZ_00044902 -->

    <owl:NamedIndividual rdf:about="http://purl.obolibrary.org/obo/GAZ_00044902">
        <obo:IAO_0000115>A reservoir in Egypt and northern Sudan created as a result of the construction of the Aswan High Dam across the waters of the Nile between 1958 and 1970. The lake is some 550 km long and 35 km across at its widest point, which is near the Tropic of Cancer. It covers a total surface area of 5,250 km2 and has a storage capacity of some 157 km2 of water.</obo:IAO_0000115>
        <oboInOwl:hasOBONamespace>GAZ</oboInOwl:hasOBONamespace>
        <oboInOwl:id>GAZ:00044902</oboInOwl:id>
        <rdfs:label>Lake Nasser</rdfs:label>
    </owl:NamedIndividual>
    


    <!-- http://purl.obolibrary.org/obo/GAZ_00048569 -->

    <owl:NamedIndividual rdf:about="http://purl.obolibrary.org/obo/GAZ_00048569">
        <obo:RO_0001025 rdf:resource="http://purl.obolibrary.org/obo/GAZ_00000654"/>
        <obo:IAO_0000115>A barren rocky island in the mouth of the Gulf of Suez in the northern Red Sea.</obo:IAO_0000115>
        <oboInOwl:hasOBONamespace>GAZ</oboInOwl:hasOBONamespace>
        <oboInOwl:id>GAZ:00048569</oboInOwl:id>
        <rdfs:label>Shadwan Island</rdfs:label>
    </owl:NamedIndividual>
    


    <!-- http://purl.obolibrary.org/obo/GAZ_00048570 -->

    <owl:NamedIndividual rdf:about="http://purl.obolibrary.org/obo/GAZ_00048570">
        <obo:RO_0001025 rdf:resource="http://purl.obolibrary.org/obo/GAZ_00000654"/>
        <obo:RO_0001025 rdf:resource="http://purl.obolibrary.org/obo/GAZ_00002456"/>
        <oboInOwl:hasOBONamespace>GAZ</oboInOwl:hasOBONamespace>
        <oboInOwl:id>GAZ:00048570</oboInOwl:id>
        <rdfs:label>Gifatin Island</rdfs:label>
    </owl:NamedIndividual>
    


    <!-- http://purl.obolibrary.org/obo/GAZ_00048571 -->

    <owl:NamedIndividual rdf:about="http://purl.obolibrary.org/obo/GAZ_00048571">
        <obo:RO_0001025 rdf:resource="http://purl.obolibrary.org/obo/GAZ_00000654"/>
        <obo:RO_0001025 rdf:resource="http://purl.obolibrary.org/obo/GAZ_00002456"/>
        <oboInOwl:hasOBONamespace>GAZ</oboInOwl:hasOBONamespace>
        <oboInOwl:id>GAZ:00048571</oboInOwl:id>
        <rdfs:label>Qeisum Island</rdfs:label>
    </owl:NamedIndividual>
    


    <!-- http://purl.obolibrary.org/obo/GAZ_00048572 -->

    <owl:NamedIndividual rdf:about="http://purl.obolibrary.org/obo/GAZ_00048572">
        <obo:RO_0001025 rdf:resource="http://purl.obolibrary.org/obo/GAZ_00000654"/>
        <obo:RO_0001025 rdf:resource="http://purl.obolibrary.org/obo/GAZ_00002456"/>
        <obo:IAO_0000115>An island in the Red Sea.</obo:IAO_0000115>
        <oboInOwl:hasOBONamespace>GAZ</oboInOwl:hasOBONamespace>
        <oboInOwl:id>GAZ:00048572</oboInOwl:id>
        <rdfs:label>Tawila Island</rdfs:label>
    </owl:NamedIndividual>
    


    <!-- http://purl.obolibrary.org/obo/GAZ_00048573 -->

    <owl:NamedIndividual rdf:about="http://purl.obolibrary.org/obo/GAZ_00048573">
        <obo:RO_0001025 rdf:resource="http://purl.obolibrary.org/obo/GAZ_00000654"/>
        <obo:RO_0001025 rdf:resource="http://purl.obolibrary.org/obo/GAZ_00002456"/>
        <oboInOwl:hasOBONamespace>GAZ</oboInOwl:hasOBONamespace>
        <oboInOwl:id>GAZ:00048573</oboInOwl:id>
        <rdfs:label>Gubal Island</rdfs:label>
    </owl:NamedIndividual>
    


    <!-- http://purl.obolibrary.org/obo/GAZ_00049003 -->

    <owl:NamedIndividual rdf:about="http://purl.obolibrary.org/obo/GAZ_00049003">
        <obo:RO_0001025 rdf:resource="http://purl.obolibrary.org/obo/GAZ_00002456"/>
        <obo:IAO_0000115>A large coral island group in the Red Sea, belonging to Saudi Arabia. It is located some 40 km offshore from Jizan, in the far southwestern part of the country.</obo:IAO_0000115>
        <oboInOwl:hasOBONamespace>GAZ</oboInOwl:hasOBONamespace>
        <oboInOwl:id>GAZ:00049003</oboInOwl:id>
        <rdfs:label>Farasan Islands</rdfs:label>
    </owl:NamedIndividual>
    


    <!-- http://purl.obolibrary.org/obo/GAZ_00049004 -->

    <owl:NamedIndividual rdf:about="http://purl.obolibrary.org/obo/GAZ_00049004">
        <obo:RO_0001025 rdf:resource="http://purl.obolibrary.org/obo/GAZ_00049003"/>
        <obo:IAO_0000115>One of the Farasan Islands in Saudi Arabia.</obo:IAO_0000115>
        <oboInOwl:hasOBONamespace>GAZ</oboInOwl:hasOBONamespace>
        <oboInOwl:id>GAZ:00049004</oboInOwl:id>
        <rdfs:label>Zufaf Island</rdfs:label>
    </owl:NamedIndividual>
    


    <!-- http://purl.obolibrary.org/obo/GAZ_00049005 -->

    <owl:NamedIndividual rdf:about="http://purl.obolibrary.org/obo/GAZ_00049005">
        <obo:RO_0001025 rdf:resource="http://purl.obolibrary.org/obo/GAZ_00049003"/>
        <obo:IAO_0000115>One of the Farasan Islands in Saudi Arabia.</obo:IAO_0000115>
        <oboInOwl:hasOBONamespace>GAZ</oboInOwl:hasOBONamespace>
        <oboInOwl:id>GAZ:00049005</oboInOwl:id>
        <rdfs:label>Sajid Island</rdfs:label>
    </owl:NamedIndividual>
    


    <!-- http://purl.obolibrary.org/obo/GAZ_00049006 -->

    <owl:NamedIndividual rdf:about="http://purl.obolibrary.org/obo/GAZ_00049006">
        <obo:RO_0001025 rdf:resource="http://purl.obolibrary.org/obo/GAZ_00049003"/>
        <obo:IAO_0000115>The largest island of the Farasan Islands, in the Red Sea. It is located some 50 km offshore from Jizan, the far southwestern part of Saudi Arabia.</obo:IAO_0000115>
        <oboInOwl:hasOBONamespace>GAZ</oboInOwl:hasOBONamespace>
        <oboInOwl:id>GAZ:00049006</oboInOwl:id>
        <rdfs:label>Farasan Island</rdfs:label>
    </owl:NamedIndividual>
    


    <!-- http://purl.obolibrary.org/obo/GAZ_00049007 -->

    <owl:NamedIndividual rdf:about="http://purl.obolibrary.org/obo/GAZ_00049007">
        <obo:RO_0001025 rdf:resource="http://purl.obolibrary.org/obo/GAZ_00007862"/>
        <obo:IAO_0000115>The narrow sea passages, about 13 km wide, between the Sinai and Arabian peninsulas which separates the Gulf of Aqaba from the Red Sea.</obo:IAO_0000115>
        <oboInOwl:hasOBONamespace>GAZ</oboInOwl:hasOBONamespace>
        <oboInOwl:id>GAZ:00049007</oboInOwl:id>
        <rdfs:label>Straits of Tiran</rdfs:label>
    </owl:NamedIndividual>
    


    <!-- http://purl.obolibrary.org/obo/GAZ_00049008 -->

    <owl:NamedIndividual rdf:about="http://purl.obolibrary.org/obo/GAZ_00049008">
        <obo:RO_0001025 rdf:resource="http://purl.obolibrary.org/obo/GAZ_00049007"/>
        <obo:RO_0001025 rdf:resource="http://purl.obolibrary.org/obo/GAZ_00089762"/>
        <obo:IAO_0000115>A Saudi Arabian island in the Straits of Tiran east of Tiran Island.</obo:IAO_0000115>
        <oboInOwl:hasOBONamespace>GAZ</oboInOwl:hasOBONamespace>
        <oboInOwl:id>GAZ:00049008</oboInOwl:id>
        <rdfs:label>Sanafir Island</rdfs:label>
    </owl:NamedIndividual>
    


    <!-- http://purl.obolibrary.org/obo/GAZ_00049009 -->

    <owl:NamedIndividual rdf:about="http://purl.obolibrary.org/obo/GAZ_00049009">
        <obo:RO_0001025 rdf:resource="http://purl.obolibrary.org/obo/GAZ_00049007"/>
        <obo:RO_0001025 rdf:resource="http://purl.obolibrary.org/obo/GAZ_00089762"/>
        <obo:IAO_0000115>An island belonging to Saudi Arabia at the entrance of the Straits of Tiran, which separates the Red Sea and the Gulf of Aqaba.</obo:IAO_0000115>
        <oboInOwl:hasOBONamespace>GAZ</oboInOwl:hasOBONamespace>
        <oboInOwl:id>GAZ:00049009</oboInOwl:id>
        <rdfs:label>Tiran Island</rdfs:label>
    </owl:NamedIndividual>
    


    <!-- http://purl.obolibrary.org/obo/GAZ_00049021 -->

    <owl:NamedIndividual rdf:about="http://purl.obolibrary.org/obo/GAZ_00049021">
        <obo:RO_0001025 rdf:resource="http://purl.obolibrary.org/obo/GAZ_00002456"/>
        <obo:IAO_0000115>An island in the Red Sea.</obo:IAO_0000115>
        <oboInOwl:hasOBONamespace>GAZ</oboInOwl:hasOBONamespace>
        <oboInOwl:id>GAZ:00049021</oboInOwl:id>
        <rdfs:label>Jazirat Antufish</rdfs:label>
    </owl:NamedIndividual>
    


    <!-- http://purl.obolibrary.org/obo/GAZ_00051094 -->

    <owl:NamedIndividual rdf:about="http://purl.obolibrary.org/obo/GAZ_00051094">
        <obo:RO_0001025 rdf:resource="http://purl.obolibrary.org/obo/GAZ_00002456"/>
        <oboInOwl:hasOBONamespace>GAZ</oboInOwl:hasOBONamespace>
        <oboInOwl:id>GAZ:00051094</oboInOwl:id>
        <rdfs:label>Strait of Gubal</rdfs:label>
    </owl:NamedIndividual>
    


    <!-- http://purl.obolibrary.org/obo/GAZ_00051196 -->

    <owl:NamedIndividual rdf:about="http://purl.obolibrary.org/obo/GAZ_00051196">
        <obo:RO_0001025 rdf:resource="http://purl.obolibrary.org/obo/GAZ_00000667"/>
        <obo:RO_0001025 rdf:resource="http://purl.obolibrary.org/obo/GAZ_00051197"/>
        <obo:IAO_0000115>A desert basin within the Libyan Desert of north-western Egypt. It is bounded by a steep, and in places precipitous, escarpment, along the northwestern and northern sides, which rises to heights of over 300 m, and a few km away from the escarpment edge, to over 500 m. By contrast the southern and eastern sides of the depression rise more gradually to the plateau of the Western Desert. Saline marshes/deserts, up to 30 km wide and over 150 km long, are situated under the escarpment along the northern side of the depression, and other marshes extend out into the southern central part of the basin.</obo:IAO_0000115>
        <oboInOwl:hasOBONamespace>GAZ</oboInOwl:hasOBONamespace>
        <oboInOwl:id>GAZ:00051196</oboInOwl:id>
        <rdfs:label>Qattara Depression</rdfs:label>
    </owl:NamedIndividual>
    


    <!-- http://purl.obolibrary.org/obo/GAZ_00051197 -->

    <owl:NamedIndividual rdf:about="http://purl.obolibrary.org/obo/GAZ_00051197">
        <obo:IAO_0000115>A desert that is located in the northern and eastern part of the Sahara Desert and occupies southwestern Egypt, eastern Libya and northwestern Sudan. Covering an area of approximately 1,100,000 km2 it extends approximately 1,100 km from east to west, and 1,000 km from north to south, in about the shape of a rectangle.</obo:IAO_0000115>
        <oboInOwl:hasOBONamespace>GAZ</oboInOwl:hasOBONamespace>
        <oboInOwl:id>GAZ:00051197</oboInOwl:id>
        <rdfs:label>Libyan Desert</rdfs:label>
    </owl:NamedIndividual>
    


    <!-- http://purl.obolibrary.org/obo/GAZ_00051198 -->

    <owl:NamedIndividual rdf:about="http://purl.obolibrary.org/obo/GAZ_00051198">
        <obo:IAO_0000115>A desert region in the south central Sahara. It comprises a vast plain of sand stretching from northeastern Niger into western Chad, occupying an area of over 400,000 km2). Its boundaries are conventionally said to be the Air Mountains in the west, the Ahaggar Mountains in the north, the Djado Plateau in the northeast, the Tibesti Mountains in the east and the basin of Lake Chad in the south.</obo:IAO_0000115>
        <oboInOwl:hasOBONamespace>GAZ</oboInOwl:hasOBONamespace>
        <oboInOwl:id>GAZ:00051198</oboInOwl:id>
        <rdfs:label>Erg of Tenere</rdfs:label>
    </owl:NamedIndividual>
    


    <!-- http://purl.obolibrary.org/obo/GAZ_00051199 -->

    <owl:NamedIndividual rdf:about="http://purl.obolibrary.org/obo/GAZ_00051199">
        <obo:RO_0001025 rdf:resource="http://purl.obolibrary.org/obo/GAZ_00051197"/>
        <obo:IAO_0000115>A sand sea.</obo:IAO_0000115>
        <oboInOwl:hasOBONamespace>GAZ</oboInOwl:hasOBONamespace>
        <oboInOwl:id>GAZ:00051199</oboInOwl:id>
        <rdfs:label>Rebiana Sand Sea</rdfs:label>
    </owl:NamedIndividual>
    


    <!-- http://purl.obolibrary.org/obo/GAZ_00051200 -->

    <owl:NamedIndividual rdf:about="http://purl.obolibrary.org/obo/GAZ_00051200">
        <obo:RO_0001025 rdf:resource="http://purl.obolibrary.org/obo/GAZ_00051197"/>
        <obo:IAO_0000115>A sand sea.</obo:IAO_0000115>
        <oboInOwl:hasOBONamespace>GAZ</oboInOwl:hasOBONamespace>
        <oboInOwl:id>GAZ:00051200</oboInOwl:id>
        <rdfs:label>Egyptian Sand Sea</rdfs:label>
    </owl:NamedIndividual>
    


    <!-- http://purl.obolibrary.org/obo/GAZ_00051201 -->

    <owl:NamedIndividual rdf:about="http://purl.obolibrary.org/obo/GAZ_00051201">
        <obo:RO_0001025 rdf:resource="http://purl.obolibrary.org/obo/GAZ_00051197"/>
        <obo:IAO_0000115>A sand sea.</obo:IAO_0000115>
        <oboInOwl:hasOBONamespace>GAZ</oboInOwl:hasOBONamespace>
        <oboInOwl:id>GAZ:00051201</oboInOwl:id>
        <rdfs:label>Kalansho Sand Sea</rdfs:label>
    </owl:NamedIndividual>
    


    <!-- http://purl.obolibrary.org/obo/GAZ_00051202 -->

    <owl:NamedIndividual rdf:about="http://purl.obolibrary.org/obo/GAZ_00051202">
        <obo:RO_0001025 rdf:resource="http://purl.obolibrary.org/obo/GAZ_00051198"/>
        <obo:IAO_0000115>A dune sea that stretches from Fachi, east of the Air Mountains in north central Niger, east past the town of Bilma, on to the Chadian border. It surrounds on three sides the oasis of Bilma, southernmost of a north south string of oasies of the Kaouar rise.</obo:IAO_0000115>
        <oboInOwl:hasOBONamespace>GAZ</oboInOwl:hasOBONamespace>
        <oboInOwl:id>GAZ:00051202</oboInOwl:id>
        <rdfs:label>Erg of Bilma</rdfs:label>
    </owl:NamedIndividual>
    


    <!-- http://purl.obolibrary.org/obo/GAZ_00051203 -->

    <owl:NamedIndividual rdf:about="http://purl.obolibrary.org/obo/GAZ_00051203">
        <obo:RO_0001025 rdf:resource="http://purl.obolibrary.org/obo/GAZ_00004033"/>
        <obo:IAO_0000115>A sand sea. An that is 22 km long (North-South) and 5 km wide. Its dunes reach a maximum height of 150 meters. It is located roughly 40 km south-east of Erfoud.</obo:IAO_0000115>
        <oboInOwl:hasOBONamespace>GAZ</oboInOwl:hasOBONamespace>
        <oboInOwl:id>GAZ:00051203</oboInOwl:id>
        <rdfs:label>Erg Chebbi</rdfs:label>
    </owl:NamedIndividual>
    


    <!-- http://purl.obolibrary.org/obo/GAZ_00051269 -->

    <owl:NamedIndividual rdf:about="http://purl.obolibrary.org/obo/GAZ_00051269">
        <obo:RO_0001025 rdf:resource="http://purl.obolibrary.org/obo/GAZ_00002456"/>
        <obo:IAO_0000115>A strait connecting the Red Sea to the Indian Ocean in the Gulf of Aden. The Yemeni island of Perim divides the strait into two channels.</obo:IAO_0000115>
        <oboInOwl:hasOBONamespace>GAZ</oboInOwl:hasOBONamespace>
        <oboInOwl:id>GAZ:00051269</oboInOwl:id>
        <rdfs:label>Bab-el-Mandeb</rdfs:label>
    </owl:NamedIndividual>
    


    <!-- http://purl.obolibrary.org/obo/GAZ_00052491 -->

    <owl:NamedIndividual rdf:about="http://purl.obolibrary.org/obo/GAZ_00052491">
        <obo:RO_0001025 rdf:resource="http://purl.obolibrary.org/obo/GAZ_00000653"/>
    </owl:NamedIndividual>
    


    <!-- http://purl.obolibrary.org/obo/GAZ_00052492 -->

    <owl:NamedIndividual rdf:about="http://purl.obolibrary.org/obo/GAZ_00052492">
        <obo:RO_0001025 rdf:resource="http://purl.obolibrary.org/obo/GAZ_00066372"/>
    </owl:NamedIndividual>
    


    <!-- http://purl.obolibrary.org/obo/GAZ_00052493 -->

    <owl:NamedIndividual rdf:about="http://purl.obolibrary.org/obo/GAZ_00052493">
        <obo:RO_0001025 rdf:resource="http://purl.obolibrary.org/obo/GAZ_00066368"/>
    </owl:NamedIndividual>
    


    <!-- http://purl.obolibrary.org/obo/GAZ_00052494 -->

    <owl:NamedIndividual rdf:about="http://purl.obolibrary.org/obo/GAZ_00052494">
        <obo:RO_0001025 rdf:resource="http://purl.obolibrary.org/obo/GAZ_00052493"/>
        <oboInOwl:hasOBONamespace>GAZ</oboInOwl:hasOBONamespace>
        <oboInOwl:id>GAZ:00052494</oboInOwl:id>
        <rdfs:label>Village of Abadii Valley</rdfs:label>
    </owl:NamedIndividual>
    


    <!-- http://purl.obolibrary.org/obo/GAZ_00052553 -->

    <owl:NamedIndividual rdf:about="http://purl.obolibrary.org/obo/GAZ_00052553">
        <obo:IAO_0000115>A river that rises in the central highlands of Ethiopia near Mount Qachen, from where it flows west, north, then west again, forming the westernmost border of Ethiopia and Eritrea. The river continues into northeastern Sudan, where at 14deg10minN, 36degE, the Tekeze joins the Atbarah River, the lower course of which is a tributary of the Nile. The Tekeze is perhaps the true upper course of the Atbarah, as the former follows the longer course prior to the confluence of the two rivers. The names of its main tributaries in Ethiopia from its source are: on the right bank Tahali, Meri, Sellare, Sullo, Arekwa, Gheoa, Wari, Firafira, Tocoro and Gumalo Rivers; on the left bank Nili, Balagas, Saha, Bembea, Ataba, Zarima, and Kwalema Rivers.</obo:IAO_0000115>
        <oboInOwl:hasOBONamespace>GAZ</oboInOwl:hasOBONamespace>
        <oboInOwl:id>GAZ:00052553</oboInOwl:id>
        <rdfs:label>Tekeze River</rdfs:label>
    </owl:NamedIndividual>
    


    <!-- http://purl.obolibrary.org/obo/GAZ_00053489 -->

    <owl:NamedIndividual rdf:about="http://purl.obolibrary.org/obo/GAZ_00053489">
        <obo:RO_0001025 rdf:resource="http://purl.obolibrary.org/obo/GAZ_00103898"/>
        <obo:IAO_0000115>A volcanic field covers a broad area of about 1050 km2 in the Tuareg shield in the southern Air region of Niger. Activity began with the eruption of about 30 trachytic and phonolitic volcanoes through Precambrian basement rocks. This was followed by the formation of about 130 basaltic cones that typically produced a valley filling lava flow. A series of NW-SE-trending faults control volcano locations.</obo:IAO_0000115>
        <oboInOwl:hasOBONamespace>GAZ</oboInOwl:hasOBONamespace>
        <oboInOwl:id>GAZ:00053489</oboInOwl:id>
        <rdfs:label>Todra Volcanic Field</rdfs:label>
    </owl:NamedIndividual>
    


    <!-- http://purl.obolibrary.org/obo/GAZ_00053496 -->

    <owl:NamedIndividual rdf:about="http://purl.obolibrary.org/obo/GAZ_00053496">
        <obo:IAO_0000115>A volcanic field that lies in the Sahara desert of south-central Libya, south of the Haruj volcanic field. A 4 km wide, 100-m-deep caldera contains a post-caldera scoria cone, Wau-en-Namus. An apron of dark basaltic tephra extends 10-20 km around the caldera in stark contrast to the light-colored desert sand prominent in satellite views. Three small saline lakes of variable color contribute to the name of the volcano.</obo:IAO_0000115>
        <oboInOwl:hasOBONamespace>GAZ</oboInOwl:hasOBONamespace>
        <oboInOwl:id>GAZ:00053496</oboInOwl:id>
        <rdfs:label>Wau-en-Namus Volcanic Field</rdfs:label>
    </owl:NamedIndividual>
    


    <!-- http://purl.obolibrary.org/obo/GAZ_00053509 -->

    <owl:NamedIndividual rdf:about="http://purl.obolibrary.org/obo/GAZ_00053509">
        <obo:RO_0001025 rdf:resource="http://purl.obolibrary.org/obo/GAZ_00057756"/>
        <obo:IAO_0000115>A volcanic field is located in the Bayuda Desert of NE Sudan, south of the major Abu Hamed bend of the Nile River about 300 km north of capital city of Khartoum. More than 90 eruptive centers along a WNW-ESE line were constructed over Precambrian and Paleozoic granitic rocks near the center of the Bayuda Desert. Most vents of the Bayuda field are cinder cones that produced lava flows which breached the cones. About 10% of vents in the field are explosion craters, the largest of which, named Hosh ed Dalam, is 1.3 km wide and up to 500 m deep.</obo:IAO_0000115>
        <oboInOwl:hasOBONamespace>GAZ</oboInOwl:hasOBONamespace>
        <oboInOwl:id>GAZ:00053509</oboInOwl:id>
        <rdfs:label>Bayuda Volcanic Field</rdfs:label>
    </owl:NamedIndividual>
    


    <!-- http://purl.obolibrary.org/obo/GAZ_00053510 -->

    <owl:NamedIndividual rdf:about="http://purl.obolibrary.org/obo/GAZ_00053510">
        <obo:RO_0001025 rdf:resource="http://purl.obolibrary.org/obo/GAZ_00053509"/>
        <obo:IAO_0000115>A volanic crater.</obo:IAO_0000115>
        <oboInOwl:hasOBONamespace>GAZ</oboInOwl:hasOBONamespace>
        <oboInOwl:id>GAZ:00053510</oboInOwl:id>
        <rdfs:label>Hosh ed Dalam</rdfs:label>
    </owl:NamedIndividual>
    


    <!-- http://purl.obolibrary.org/obo/GAZ_00053511 -->

    <owl:NamedIndividual rdf:about="http://purl.obolibrary.org/obo/GAZ_00053511">
        <obo:RO_0001025 rdf:resource="http://purl.obolibrary.org/obo/GAZ_00057756"/>
        <obo:IAO_0000115>A volcanic field (shield volcano) located in the Bayuda desert of NE Sudan, immediately west of the Nile River, NE of the capital city of Khartoum. Jebel Umm Arafieb consists of a low-angle shield volcano of basanitic-to-trachybasaltic composition formed of several overlapping aa lava flows erupted from a vent now capped by a spatter cone.</obo:IAO_0000115>
        <oboInOwl:hasOBONamespace>GAZ</oboInOwl:hasOBONamespace>
        <oboInOwl:id>GAZ:00053511</oboInOwl:id>
        <rdfs:label>Jebel Umm Arafieb Volcanic Field</rdfs:label>
    </owl:NamedIndividual>
    


    <!-- http://purl.obolibrary.org/obo/GAZ_00053592 -->

    <owl:NamedIndividual rdf:about="http://purl.obolibrary.org/obo/GAZ_00053592">
        <obo:RO_0001025 rdf:resource="http://purl.obolibrary.org/obo/GAZ_00002456"/>
        <obo:IAO_0000115>A stratovolcano rises from a 1200 m depth in the south-central Red Sea, forming an oval-shaped island about 3 km long. Located northwest of the constricted Bab al-Mandab passage at the mouth of the Red Sea, about half way between Yemen and Eritrea.</obo:IAO_0000115>
        <oboInOwl:hasOBONamespace>GAZ</oboInOwl:hasOBONamespace>
        <oboInOwl:id>GAZ:00053592</oboInOwl:id>
        <rdfs:label>Jabal al-Tair Island</rdfs:label>
    </owl:NamedIndividual>
    


    <!-- http://purl.obolibrary.org/obo/GAZ_00053593 -->

    <owl:NamedIndividual rdf:about="http://purl.obolibrary.org/obo/GAZ_00053593">
        <obo:RO_0001025 rdf:resource="http://purl.obolibrary.org/obo/GAZ_00053592"/>
        <obo:IAO_0000115>A volcanic vent.</obo:IAO_0000115>
        <oboInOwl:hasOBONamespace>GAZ</oboInOwl:hasOBONamespace>
        <oboInOwl:id>GAZ:00053593</oboInOwl:id>
        <rdfs:label>Jebel Duchan</rdfs:label>
    </owl:NamedIndividual>
    


    <!-- http://purl.obolibrary.org/obo/GAZ_00053594 -->

    <owl:NamedIndividual rdf:about="http://purl.obolibrary.org/obo/GAZ_00053594">
        <obo:RO_0001025 rdf:resource="http://purl.obolibrary.org/obo/GAZ_00002456"/>
        <obo:IAO_0000115>The largest of a group of 10 small islands and submerged shoals that rise from a shallow platform in the Red Sea rift.</obo:IAO_0000115>
        <oboInOwl:hasOBONamespace>GAZ</oboInOwl:hasOBONamespace>
        <oboInOwl:id>GAZ:00053594</oboInOwl:id>
        <rdfs:label>Jebel Zubair</rdfs:label>
    </owl:NamedIndividual>
    


    <!-- http://purl.obolibrary.org/obo/GAZ_00053595 -->

    <owl:NamedIndividual rdf:about="http://purl.obolibrary.org/obo/GAZ_00053595">
        <obo:RO_0001025 rdf:resource="http://purl.obolibrary.org/obo/GAZ_00005876"/>
        <obo:IAO_0000115>The largest of the Hanish Islands, which belong to Yemen.</obo:IAO_0000115>
        <oboInOwl:hasOBONamespace>GAZ</oboInOwl:hasOBONamespace>
        <oboInOwl:id>GAZ:00053595</oboInOwl:id>
        <rdfs:label>Great Hanish Island</rdfs:label>
    </owl:NamedIndividual>
    


    <!-- http://purl.obolibrary.org/obo/GAZ_00053596 -->

    <owl:NamedIndividual rdf:about="http://purl.obolibrary.org/obo/GAZ_00053596">
        <obo:RO_0001025 rdf:resource="http://purl.obolibrary.org/obo/GAZ_00005876"/>
        <oboInOwl:hasOBONamespace>GAZ</oboInOwl:hasOBONamespace>
        <oboInOwl:id>GAZ:00053596</oboInOwl:id>
        <rdfs:label>Little Hanish Island</rdfs:label>
    </owl:NamedIndividual>
    


    <!-- http://purl.obolibrary.org/obo/GAZ_00053597 -->

    <owl:NamedIndividual rdf:about="http://purl.obolibrary.org/obo/GAZ_00053597">
        <obo:RO_0001025 rdf:resource="http://purl.obolibrary.org/obo/GAZ_00002456"/>
        <oboInOwl:hasOBONamespace>GAZ</oboInOwl:hasOBONamespace>
        <oboInOwl:id>GAZ:00053597</oboInOwl:id>
        <rdfs:label>Zukur-Hanish island group</rdfs:label>
    </owl:NamedIndividual>
    


    <!-- http://purl.obolibrary.org/obo/GAZ_00057756 -->

    <owl:NamedIndividual rdf:about="http://purl.obolibrary.org/obo/GAZ_00057756">
        <obo:IAO_0000115>A desert located north of Khartoum, Sudan, west of Kadabas, and north of the Nubian Desert, together making up part of the Sahara&apos;s eastern flank.</obo:IAO_0000115>
        <oboInOwl:hasOBONamespace>GAZ</oboInOwl:hasOBONamespace>
        <oboInOwl:id>GAZ:00057756</oboInOwl:id>
        <rdfs:label>Bayuda Desert</rdfs:label>
    </owl:NamedIndividual>
    


    <!-- http://purl.obolibrary.org/obo/GAZ_00057757 -->

    <owl:NamedIndividual rdf:about="http://purl.obolibrary.org/obo/GAZ_00057757">
        <obo:IAO_0000115>The eastern region of the Sahara Desert, it spans 50, 000 km2 of northeastern Sudan between the Nile and the Red Sea.</obo:IAO_0000115>
        <oboInOwl:hasOBONamespace>GAZ</oboInOwl:hasOBONamespace>
        <oboInOwl:id>GAZ:00057757</oboInOwl:id>
        <rdfs:label>Nubian Desert</rdfs:label>
    </owl:NamedIndividual>
    


    <!-- http://purl.obolibrary.org/obo/GAZ_00057759 -->

    <owl:NamedIndividual rdf:about="http://purl.obolibrary.org/obo/GAZ_00057759">
        <obo:IAO_0000115>A desert east of the river Nile, between the Nile and the Red Sea. It extends from Egypt in the north to Eritrea in the south, and also comprises parts of Sudan and Ethiopia.</obo:IAO_0000115>
        <oboInOwl:hasOBONamespace>GAZ</oboInOwl:hasOBONamespace>
        <oboInOwl:id>GAZ:00057759</oboInOwl:id>
        <rdfs:label>Eastern Desert</rdfs:label>
    </owl:NamedIndividual>
    


    <!-- http://purl.obolibrary.org/obo/GAZ_00058791 -->

    <owl:NamedIndividual rdf:about="http://purl.obolibrary.org/obo/GAZ_00058791">
        <obo:IAO_0000115>A polymictic shallow lake complex of Uganda, about 1,720 km2 in area and at an elevation of 914 m. The Victoria Nile flows through the lake on its way from Lake Victoria to Lake Albert. The main inflow from Lake Victoria is regulated by the Nalubaale Power Station in Jinja. Another source of water is the Mount Elgon region on the border between Uganda and Kenya.</obo:IAO_0000115>
        <oboInOwl:hasOBONamespace>GAZ</oboInOwl:hasOBONamespace>
        <oboInOwl:id>GAZ:00058791</oboInOwl:id>
        <rdfs:label>Lake Kyoga</rdfs:label>
    </owl:NamedIndividual>
    


    <!-- http://purl.obolibrary.org/obo/GAZ_00058842 -->

    <owl:NamedIndividual rdf:about="http://purl.obolibrary.org/obo/GAZ_00058842">
        <obo:RO_0001025 rdf:resource="http://purl.obolibrary.org/obo/GAZ_00058843"/>
        <obo:IAO_0000115>A salt water lake between the north and south part of the Suez Canal.</obo:IAO_0000115>
        <oboInOwl:hasOBONamespace>GAZ</oboInOwl:hasOBONamespace>
        <oboInOwl:id>GAZ:00058842</oboInOwl:id>
        <rdfs:label>Great Bitter Lake</rdfs:label>
    </owl:NamedIndividual>
    


    <!-- http://purl.obolibrary.org/obo/GAZ_00058843 -->

    <owl:NamedIndividual rdf:about="http://purl.obolibrary.org/obo/GAZ_00058843">
        <obo:RO_0001025 rdf:resource="http://purl.obolibrary.org/obo/GAZ_00003934"/>
        <obo:IAO_0000115>A large artificial canal in Egypt, west of the Sinai Peninsula. It is 163 km long and 300 m wide at its narrowest point, and runs between Port Said on the Mediterranean Sea, and Suez (al-Suways) on the Red Sea. The canal comprises seven parts, north and south of the Great Bitter Lake, linking the Mediterranean Sea to the Gulf of Suez on the Red Sea.</obo:IAO_0000115>
        <oboInOwl:hasOBONamespace>GAZ</oboInOwl:hasOBONamespace>
        <oboInOwl:id>GAZ:00058843</oboInOwl:id>
        <rdfs:label>Suez Canal</rdfs:label>
    </owl:NamedIndividual>
    


    <!-- http://purl.obolibrary.org/obo/GAZ_00058844 -->

    <owl:NamedIndividual rdf:about="http://purl.obolibrary.org/obo/GAZ_00058844">
        <obo:RO_0001025 rdf:resource="http://purl.obolibrary.org/obo/GAZ_00058843"/>
        <oboInOwl:hasOBONamespace>GAZ</oboInOwl:hasOBONamespace>
        <oboInOwl:id>GAZ:00058844</oboInOwl:id>
        <rdfs:label>Little Bitter Lake</rdfs:label>
    </owl:NamedIndividual>
    


    <!-- http://purl.obolibrary.org/obo/GAZ_00058845 -->

    <owl:NamedIndividual rdf:about="http://purl.obolibrary.org/obo/GAZ_00058845">
        <obo:RO_0001025 rdf:resource="http://purl.obolibrary.org/obo/GAZ_00089767"/>
        <obo:IAO_0000115>A salt water lake in northeastern Egypt, near Port Said.</obo:IAO_0000115>
        <oboInOwl:hasOBONamespace>GAZ</oboInOwl:hasOBONamespace>
        <oboInOwl:id>GAZ:00058845</oboInOwl:id>
        <rdfs:label>Bahra el Manzala</rdfs:label>
    </owl:NamedIndividual>
    


    <!-- http://purl.obolibrary.org/obo/GAZ_00058847 -->

    <owl:NamedIndividual rdf:about="http://purl.obolibrary.org/obo/GAZ_00058847">
        <obo:RO_0001025 rdf:resource="http://purl.obolibrary.org/obo/GAZ_00000653"/>
        <obo:IAO_0000115>A saline, or rather brackish, lake with an area of about 250 km2 in northern Egypt. It is separated from the Mediterranean Sea by the narrow isthmus on which the city of Alexandria was built.</obo:IAO_0000115>
        <oboInOwl:hasOBONamespace>GAZ</oboInOwl:hasOBONamespace>
        <oboInOwl:id>GAZ:00058847</oboInOwl:id>
        <rdfs:label>Bahra el Maryut</rdfs:label>
    </owl:NamedIndividual>
    


    <!-- http://purl.obolibrary.org/obo/GAZ_00058848 -->

    <owl:NamedIndividual rdf:about="http://purl.obolibrary.org/obo/GAZ_00058848">
        <obo:RO_0001025 rdf:resource="http://purl.obolibrary.org/obo/GAZ_00089774"/>
        <obo:IAO_0000115>An endorheic saline lake; the remnant of Lake Moeris. Located in the northwest of the Faiyum Oasis, 80 km southwest of Cairo. In the past artificially fed by water from the Nile, but now, with modern agricultural practices, it receives only the run-off from the irrigated peripheral lands. This enters the lake via two canals at the eastern end.</obo:IAO_0000115>
        <oboInOwl:hasOBONamespace>GAZ</oboInOwl:hasOBONamespace>
        <oboInOwl:id>GAZ:00058848</oboInOwl:id>
        <rdfs:label>Birket Qarun</rdfs:label>
    </owl:NamedIndividual>
    


    <!-- http://purl.obolibrary.org/obo/GAZ_00058849 -->

    <owl:NamedIndividual rdf:about="http://purl.obolibrary.org/obo/GAZ_00058849">
        <obo:RO_0001025 rdf:resource="http://purl.obolibrary.org/obo/GAZ_00000645"/>
        <obo:RO_0001025 rdf:resource="http://purl.obolibrary.org/obo/GAZ_00051197"/>
        <obo:IAO_0000115>Recently formed endorheic lakes in the Sahara Desert of Egypt. Caused by water from Lake Nasser running through the Sadat Canal.</obo:IAO_0000115>
        <oboInOwl:hasOBONamespace>GAZ</oboInOwl:hasOBONamespace>
        <oboInOwl:id>GAZ:00058849</oboInOwl:id>
        <rdfs:label>Toshka Lakes</rdfs:label>
    </owl:NamedIndividual>
    


    <!-- http://purl.obolibrary.org/obo/GAZ_00058851 -->

    <owl:NamedIndividual rdf:about="http://purl.obolibrary.org/obo/GAZ_00058851">
        <obo:RO_0001025 rdf:resource="http://purl.obolibrary.org/obo/GAZ_00000664"/>
        <obo:RO_0001025 rdf:resource="http://purl.obolibrary.org/obo/GAZ_00058843"/>
        <obo:IAO_0000115>A lake. Located within a depression that spans the isthmus between the Red Sea and the Mediterranean Sea.</obo:IAO_0000115>
        <oboInOwl:hasOBONamespace>GAZ</oboInOwl:hasOBONamespace>
        <oboInOwl:id>GAZ:00058851</oboInOwl:id>
        <rdfs:label>Lake Timsah</rdfs:label>
    </owl:NamedIndividual>
    


    <!-- http://purl.obolibrary.org/obo/GAZ_00058872 -->

    <owl:NamedIndividual rdf:about="http://purl.obolibrary.org/obo/GAZ_00058872">
        <obo:IAO_0000115>The two dams at the first cataract on the Nile in Egypt.</obo:IAO_0000115>
        <oboInOwl:hasOBONamespace>GAZ</oboInOwl:hasOBONamespace>
        <oboInOwl:id>GAZ:00058872</oboInOwl:id>
        <rdfs:label>Aswan Dams</rdfs:label>
    </owl:NamedIndividual>
    


    <!-- http://purl.obolibrary.org/obo/GAZ_00058873 -->

    <owl:NamedIndividual rdf:about="http://purl.obolibrary.org/obo/GAZ_00058873">
        <obo:RO_0001025 rdf:resource="http://purl.obolibrary.org/obo/GAZ_00058872"/>
        <obo:IAO_0000115>The newer of the Aswan Dams, completed in 1968. It is located 7 km south of Aswan City.</obo:IAO_0000115>
        <oboInOwl:hasOBONamespace>GAZ</oboInOwl:hasOBONamespace>
        <oboInOwl:id>GAZ:00058873</oboInOwl:id>
        <rdfs:label>Aswan High Dam</rdfs:label>
    </owl:NamedIndividual>
    


    <!-- http://purl.obolibrary.org/obo/GAZ_00058874 -->

    <owl:NamedIndividual rdf:about="http://purl.obolibrary.org/obo/GAZ_00058874">
        <obo:RO_0001025 rdf:resource="http://purl.obolibrary.org/obo/GAZ_00058872"/>
        <obo:IAO_0000115>The first of the Aswan Dams on the Nile, finished in 1902.</obo:IAO_0000115>
        <oboInOwl:hasOBONamespace>GAZ</oboInOwl:hasOBONamespace>
        <oboInOwl:id>GAZ:00058874</oboInOwl:id>
        <rdfs:label>Aswan Low Dam</rdfs:label>
    </owl:NamedIndividual>
    


    <!-- http://purl.obolibrary.org/obo/GAZ_00058877 -->

    <owl:NamedIndividual rdf:about="http://purl.obolibrary.org/obo/GAZ_00058877">
        <obo:RO_0001025 rdf:resource="http://purl.obolibrary.org/obo/GAZ_00009949"/>
        <obo:IAO_0000115>A dam that was completed in 1862. Its purpose was to improve irrigation in the Nile Delta area of Egypt.</obo:IAO_0000115>
        <oboInOwl:hasOBONamespace>GAZ</oboInOwl:hasOBONamespace>
        <oboInOwl:id>GAZ:00058877</oboInOwl:id>
        <rdfs:label>Delta Barrage</rdfs:label>
    </owl:NamedIndividual>
    


    <!-- http://purl.obolibrary.org/obo/GAZ_00058878 -->

    <owl:NamedIndividual rdf:about="http://purl.obolibrary.org/obo/GAZ_00058878">
        <rdf:type rdf:resource="http://purl.obolibrary.org/obo/ENVO_00000074"/>
        <obo:IAO_0000115>A barrage on the River Nile in Egypt.</obo:IAO_0000115>
        <oboInOwl:hasOBONamespace>GAZ</oboInOwl:hasOBONamespace>
        <oboInOwl:id>GAZ:00058878</oboInOwl:id>
        <rdfs:label>Esna Barrage</rdfs:label>
    </owl:NamedIndividual>
    


    <!-- http://purl.obolibrary.org/obo/GAZ_00058879 -->

    <owl:NamedIndividual rdf:about="http://purl.obolibrary.org/obo/GAZ_00058879">
        <rdf:type rdf:resource="http://purl.obolibrary.org/obo/ENVO_00000074"/>
        <obo:IAO_0000115>A barrage on the River Nile in Egypt.</obo:IAO_0000115>
        <oboInOwl:hasOBONamespace>GAZ</oboInOwl:hasOBONamespace>
        <oboInOwl:id>GAZ:00058879</oboInOwl:id>
        <rdfs:label>Nag Hammadi Barrage</rdfs:label>
    </owl:NamedIndividual>
    


    <!-- http://purl.obolibrary.org/obo/GAZ_00058880 -->

    <owl:NamedIndividual rdf:about="http://purl.obolibrary.org/obo/GAZ_00058880">
        <rdf:type rdf:resource="http://purl.obolibrary.org/obo/ENVO_00000074"/>
        <obo:IAO_0000115>A barrage on the River Nile in Egypt.</obo:IAO_0000115>
        <oboInOwl:hasOBONamespace>GAZ</oboInOwl:hasOBONamespace>
        <oboInOwl:id>GAZ:00058880</oboInOwl:id>
        <rdfs:label>Assuit Barrage</rdfs:label>
    </owl:NamedIndividual>
    


    <!-- http://purl.obolibrary.org/obo/GAZ_00058881 -->

    <owl:NamedIndividual rdf:about="http://purl.obolibrary.org/obo/GAZ_00058881">
        <obo:IAO_0000115>A dam on the Rosetta Canal.</obo:IAO_0000115>
        <oboInOwl:hasOBONamespace>GAZ</oboInOwl:hasOBONamespace>
        <oboInOwl:id>GAZ:00058881</oboInOwl:id>
        <rdfs:label>Edfina Barrage</rdfs:label>
    </owl:NamedIndividual>
    


    <!-- http://purl.obolibrary.org/obo/GAZ_00058882 -->

    <owl:NamedIndividual rdf:about="http://purl.obolibrary.org/obo/GAZ_00058882">
        <obo:IAO_0000115>A dam on the Damietta Canal.</obo:IAO_0000115>
        <oboInOwl:hasOBONamespace>GAZ</oboInOwl:hasOBONamespace>
        <oboInOwl:id>GAZ:00058882</oboInOwl:id>
        <rdfs:label>Faraskour Barrage</rdfs:label>
    </owl:NamedIndividual>
    


    <!-- http://purl.obolibrary.org/obo/GAZ_00058883 -->

    <owl:NamedIndividual rdf:about="http://purl.obolibrary.org/obo/GAZ_00058883">
        <obo:IAO_0000115>A dam on the Damietta Canal.</obo:IAO_0000115>
        <oboInOwl:hasOBONamespace>GAZ</oboInOwl:hasOBONamespace>
        <oboInOwl:id>GAZ:00058883</oboInOwl:id>
        <rdfs:label>Zitta Barrage</rdfs:label>
    </owl:NamedIndividual>
    


    <!-- http://purl.obolibrary.org/obo/GAZ_00058884 -->

    <owl:NamedIndividual rdf:about="http://purl.obolibrary.org/obo/GAZ_00058884"/>
    


    <!-- http://purl.obolibrary.org/obo/GAZ_00058886 -->

    <owl:NamedIndividual rdf:about="http://purl.obolibrary.org/obo/GAZ_00058886"/>
    


    <!-- http://purl.obolibrary.org/obo/GAZ_00058890 -->

    <owl:NamedIndividual rdf:about="http://purl.obolibrary.org/obo/GAZ_00058890"/>
    


    <!-- http://purl.obolibrary.org/obo/GAZ_00058891 -->

    <owl:NamedIndividual rdf:about="http://purl.obolibrary.org/obo/GAZ_00058891">
        <obo:RO_0001025 rdf:resource="http://purl.obolibrary.org/obo/GAZ_00058886"/>
        <obo:IAO_0000115>An island in the River Nile in Egypt near the Fourth Cataract in Dar al-Manasir.</obo:IAO_0000115>
        <oboInOwl:hasOBONamespace>GAZ</oboInOwl:hasOBONamespace>
        <oboInOwl:id>GAZ:00058891</oboInOwl:id>
        <rdfs:label>Island of Muqrat</rdfs:label>
    </owl:NamedIndividual>
    


    <!-- http://purl.obolibrary.org/obo/GAZ_00058892 -->

    <owl:NamedIndividual rdf:about="http://purl.obolibrary.org/obo/GAZ_00058892">
        <obo:IAO_0000115>A dam under construction on the River Nile in Sudan, about 350 km north of the capital Khartoum.</obo:IAO_0000115>
        <oboInOwl:hasOBONamespace>GAZ</oboInOwl:hasOBONamespace>
        <oboInOwl:id>GAZ:00058892</oboInOwl:id>
        <rdfs:label>Merowe High Dam</rdfs:label>
    </owl:NamedIndividual>
    


    <!-- http://purl.obolibrary.org/obo/GAZ_00066359 -->

    <owl:NamedIndividual rdf:about="http://purl.obolibrary.org/obo/GAZ_00066359">
        <obo:RO_0001025 rdf:resource="http://purl.obolibrary.org/obo/GAZ_00000653"/>
        <obo:IAO_0000115>An administrative region (kism) of Alexandria Governorate.</obo:IAO_0000115>
        <oboInOwl:hasOBONamespace>GAZ</oboInOwl:hasOBONamespace>
        <oboInOwl:id>GAZ:00066359</oboInOwl:id>
        <rdfs:label>Kism Burj al &apos;Arab</rdfs:label>
    </owl:NamedIndividual>
    


    <!-- http://purl.obolibrary.org/obo/GAZ_00066362 -->

    <owl:NamedIndividual rdf:about="http://purl.obolibrary.org/obo/GAZ_00066362">
        <obo:RO_0001025 rdf:resource="http://purl.obolibrary.org/obo/GAZ_00052491"/>
        <obo:IAO_0000115>An urban district (hai) of Alexandria.</obo:IAO_0000115>
        <oboInOwl:hasOBONamespace>GAZ</oboInOwl:hasOBONamespace>
        <oboInOwl:id>GAZ:00066362</oboInOwl:id>
        <rdfs:label>Agami hai</rdfs:label>
    </owl:NamedIndividual>
    


    <!-- http://purl.obolibrary.org/obo/GAZ_00066363 -->

    <owl:NamedIndividual rdf:about="http://purl.obolibrary.org/obo/GAZ_00066363">
        <obo:RO_0001025 rdf:resource="http://purl.obolibrary.org/obo/GAZ_00052491"/>
        <obo:IAO_0000115>An urban district (hai) of Alexandria.</obo:IAO_0000115>
        <oboInOwl:hasOBONamespace>GAZ</oboInOwl:hasOBONamespace>
        <oboInOwl:id>GAZ:00066363</oboInOwl:id>
        <rdfs:label>al-Gomrok hai</rdfs:label>
    </owl:NamedIndividual>
    


    <!-- http://purl.obolibrary.org/obo/GAZ_00066364 -->

    <owl:NamedIndividual rdf:about="http://purl.obolibrary.org/obo/GAZ_00066364">
        <obo:RO_0001025 rdf:resource="http://purl.obolibrary.org/obo/GAZ_00052491"/>
        <obo:IAO_0000115>An urban district (hai) of Alexandria.</obo:IAO_0000115>
        <oboInOwl:hasOBONamespace>GAZ</oboInOwl:hasOBONamespace>
        <oboInOwl:id>GAZ:00066364</oboInOwl:id>
        <rdfs:label>al-Montaza hai</rdfs:label>
    </owl:NamedIndividual>
    


    <!-- http://purl.obolibrary.org/obo/GAZ_00066365 -->

    <owl:NamedIndividual rdf:about="http://purl.obolibrary.org/obo/GAZ_00066365">
        <obo:RO_0001025 rdf:resource="http://purl.obolibrary.org/obo/GAZ_00052491"/>
        <obo:IAO_0000115>An urban district (hai) of Alexandria.</obo:IAO_0000115>
        <oboInOwl:hasOBONamespace>GAZ</oboInOwl:hasOBONamespace>
        <oboInOwl:id>GAZ:00066365</oboInOwl:id>
        <rdfs:label>al-Amriya hai</rdfs:label>
    </owl:NamedIndividual>
    


    <!-- http://purl.obolibrary.org/obo/GAZ_00066366 -->

    <owl:NamedIndividual rdf:about="http://purl.obolibrary.org/obo/GAZ_00066366">
        <obo:RO_0001025 rdf:resource="http://purl.obolibrary.org/obo/GAZ_00052491"/>
        <obo:IAO_0000115>An urban district (hai) of Alexandria.</obo:IAO_0000115>
        <oboInOwl:hasOBONamespace>GAZ</oboInOwl:hasOBONamespace>
        <oboInOwl:id>GAZ:00066366</oboInOwl:id>
        <rdfs:label>Sharak hai</rdfs:label>
    </owl:NamedIndividual>
    


    <!-- http://purl.obolibrary.org/obo/GAZ_00066367 -->

    <owl:NamedIndividual rdf:about="http://purl.obolibrary.org/obo/GAZ_00066367">
        <obo:RO_0001025 rdf:resource="http://purl.obolibrary.org/obo/GAZ_00052491"/>
        <obo:IAO_0000115>An urban district (hai) of Alexandria.</obo:IAO_0000115>
        <oboInOwl:hasOBONamespace>GAZ</oboInOwl:hasOBONamespace>
        <oboInOwl:id>GAZ:00066367</oboInOwl:id>
        <rdfs:label>Wassat hai</rdfs:label>
    </owl:NamedIndividual>
    


    <!-- http://purl.obolibrary.org/obo/GAZ_00066368 -->

    <owl:NamedIndividual rdf:about="http://purl.obolibrary.org/obo/GAZ_00066368">
        <obo:RO_0001025 rdf:resource="http://purl.obolibrary.org/obo/GAZ_00000645"/>
        <obo:IAO_0000115>An administrative region (markaz) of Aswan Governorate.</obo:IAO_0000115>
        <oboInOwl:hasOBONamespace>GAZ</oboInOwl:hasOBONamespace>
        <oboInOwl:id>GAZ:00066368</oboInOwl:id>
        <rdfs:label>Edfou Region</rdfs:label>
    </owl:NamedIndividual>
    


    <!-- http://purl.obolibrary.org/obo/GAZ_00066369 -->

    <owl:NamedIndividual rdf:about="http://purl.obolibrary.org/obo/GAZ_00066369">
        <obo:RO_0001025 rdf:resource="http://purl.obolibrary.org/obo/GAZ_00000645"/>
        <obo:IAO_0000115>An administrative region (markaz) of Aswan Governorate.</obo:IAO_0000115>
        <oboInOwl:hasOBONamespace>GAZ</oboInOwl:hasOBONamespace>
        <oboInOwl:id>GAZ:00066369</oboInOwl:id>
        <rdfs:label>Nasr Region</rdfs:label>
    </owl:NamedIndividual>
    


    <!-- http://purl.obolibrary.org/obo/GAZ_00066370 -->

    <owl:NamedIndividual rdf:about="http://purl.obolibrary.org/obo/GAZ_00066370">
        <obo:RO_0001025 rdf:resource="http://purl.obolibrary.org/obo/GAZ_00000645"/>
        <obo:IAO_0000115>An administrative region (markaz) of Aswan Governorate.</obo:IAO_0000115>
        <oboInOwl:hasOBONamespace>GAZ</oboInOwl:hasOBONamespace>
        <oboInOwl:id>GAZ:00066370</oboInOwl:id>
        <rdfs:label>Draw Region</rdfs:label>
    </owl:NamedIndividual>
    


    <!-- http://purl.obolibrary.org/obo/GAZ_00066371 -->

    <owl:NamedIndividual rdf:about="http://purl.obolibrary.org/obo/GAZ_00066371">
        <obo:RO_0001025 rdf:resource="http://purl.obolibrary.org/obo/GAZ_00000645"/>
        <obo:IAO_0000115>An administrative region (markaz) of Aswan Governorate.</obo:IAO_0000115>
        <oboInOwl:hasOBONamespace>GAZ</oboInOwl:hasOBONamespace>
        <oboInOwl:id>GAZ:00066371</oboInOwl:id>
        <rdfs:label>Kom Ombou Region</rdfs:label>
    </owl:NamedIndividual>
    


    <!-- http://purl.obolibrary.org/obo/GAZ_00066372 -->

    <owl:NamedIndividual rdf:about="http://purl.obolibrary.org/obo/GAZ_00066372">
        <obo:RO_0001025 rdf:resource="http://purl.obolibrary.org/obo/GAZ_00000645"/>
        <obo:IAO_0000115>An administrative region (markaz) of Aswan Governorate.</obo:IAO_0000115>
        <oboInOwl:hasOBONamespace>GAZ</oboInOwl:hasOBONamespace>
        <oboInOwl:id>GAZ:00066372</oboInOwl:id>
        <rdfs:label>Aswan Region</rdfs:label>
    </owl:NamedIndividual>
    


    <!-- http://purl.obolibrary.org/obo/GAZ_00066373 -->

    <owl:NamedIndividual rdf:about="http://purl.obolibrary.org/obo/GAZ_00066373">
        <obo:RO_0001025 rdf:resource="http://purl.obolibrary.org/obo/GAZ_00000646"/>
        <obo:IAO_0000115>An administrative region (markaz) of Asyut Governorate.</obo:IAO_0000115>
        <oboInOwl:hasOBONamespace>GAZ</oboInOwl:hasOBONamespace>
        <oboInOwl:id>GAZ:00066373</oboInOwl:id>
        <rdfs:label>Albadary Region</rdfs:label>
    </owl:NamedIndividual>
    


    <!-- http://purl.obolibrary.org/obo/GAZ_00066374 -->

    <owl:NamedIndividual rdf:about="http://purl.obolibrary.org/obo/GAZ_00066374">
        <obo:RO_0001025 rdf:resource="http://purl.obolibrary.org/obo/GAZ_00000646"/>
        <obo:IAO_0000115>An administrative region (markaz) of Asyut Governorate.</obo:IAO_0000115>
        <oboInOwl:hasOBONamespace>GAZ</oboInOwl:hasOBONamespace>
        <oboInOwl:id>GAZ:00066374</oboInOwl:id>
        <rdfs:label>Alqousyah Region</rdfs:label>
    </owl:NamedIndividual>
    


    <!-- http://purl.obolibrary.org/obo/GAZ_00066375 -->

    <owl:NamedIndividual rdf:about="http://purl.obolibrary.org/obo/GAZ_00066375">
        <obo:RO_0001025 rdf:resource="http://purl.obolibrary.org/obo/GAZ_00000646"/>
        <obo:IAO_0000115>An administrative region (markaz) of Asyut Governorate.</obo:IAO_0000115>
        <oboInOwl:hasOBONamespace>GAZ</oboInOwl:hasOBONamespace>
        <oboInOwl:id>GAZ:00066375</oboInOwl:id>
        <rdfs:label>Alghanaiem Region</rdfs:label>
    </owl:NamedIndividual>
    


    <!-- http://purl.obolibrary.org/obo/GAZ_00066378 -->

    <owl:NamedIndividual rdf:about="http://purl.obolibrary.org/obo/GAZ_00066378">
        <obo:RO_0001025 rdf:resource="http://purl.obolibrary.org/obo/GAZ_00000646"/>
        <obo:IAO_0000115>An administrative region (markaz) of Asyut Governorate.</obo:IAO_0000115>
        <oboInOwl:hasOBONamespace>GAZ</oboInOwl:hasOBONamespace>
        <oboInOwl:id>GAZ:00066378</oboInOwl:id>
        <rdfs:label>Alfath Region</rdfs:label>
    </owl:NamedIndividual>
    


    <!-- http://purl.obolibrary.org/obo/GAZ_00066379 -->

    <owl:NamedIndividual rdf:about="http://purl.obolibrary.org/obo/GAZ_00066379">
        <obo:RO_0001025 rdf:resource="http://purl.obolibrary.org/obo/GAZ_00000655"/>
        <obo:IAO_0000115>An administrative region (markuz) of Beheira Governorate.</obo:IAO_0000115>
        <oboInOwl:hasOBONamespace>GAZ</oboInOwl:hasOBONamespace>
        <oboInOwl:id>GAZ:00066379</oboInOwl:id>
        <rdfs:label>Abou Homos Region</rdfs:label>
    </owl:NamedIndividual>
    


    <!-- http://purl.obolibrary.org/obo/GAZ_00066380 -->

    <owl:NamedIndividual rdf:about="http://purl.obolibrary.org/obo/GAZ_00066380">
        <obo:RO_0001025 rdf:resource="http://purl.obolibrary.org/obo/GAZ_00000647"/>
        <obo:IAO_0000115>An administrative region (markaz) of Beni Suef Governorate.</obo:IAO_0000115>
        <oboInOwl:hasOBONamespace>GAZ</oboInOwl:hasOBONamespace>
        <oboInOwl:id>GAZ:00066380</oboInOwl:id>
        <rdfs:label>Bani Sweif Region</rdfs:label>
    </owl:NamedIndividual>
    


    <!-- http://purl.obolibrary.org/obo/GAZ_00066381 -->

    <owl:NamedIndividual rdf:about="http://purl.obolibrary.org/obo/GAZ_00066381">
        <obo:RO_0001025 rdf:resource="http://purl.obolibrary.org/obo/GAZ_00230304"/>
        <obo:IAO_0000115>An administrative region (kism) of Helwan Governorate.</obo:IAO_0000115>
        <oboInOwl:hasOBONamespace>GAZ</oboInOwl:hasOBONamespace>
        <oboInOwl:id>GAZ:00066381</oboInOwl:id>
        <rdfs:label>Kism 15 May</rdfs:label>
    </owl:NamedIndividual>
    


    <!-- http://purl.obolibrary.org/obo/GAZ_00066382 -->

    <owl:NamedIndividual rdf:about="http://purl.obolibrary.org/obo/GAZ_00066382">
        <obo:RO_0001025 rdf:resource="http://purl.obolibrary.org/obo/GAZ_00000656"/>
        <obo:IAO_0000115>An administrative region (kisim) of Dakahlia Governorate.</obo:IAO_0000115>
        <oboInOwl:hasOBONamespace>GAZ</oboInOwl:hasOBONamespace>
        <oboInOwl:id>GAZ:00066382</oboInOwl:id>
        <rdfs:label>Gamasa Region</rdfs:label>
    </owl:NamedIndividual>
    


    <!-- http://purl.obolibrary.org/obo/GAZ_00066383 -->

    <owl:NamedIndividual rdf:about="http://purl.obolibrary.org/obo/GAZ_00066383">
        <obo:RO_0001025 rdf:resource="http://purl.obolibrary.org/obo/GAZ_00000656"/>
        <obo:IAO_0000115>An administrative region (markaz) of Dakahlia Governorate.</obo:IAO_0000115>
        <oboInOwl:hasOBONamespace>GAZ</oboInOwl:hasOBONamespace>
        <oboInOwl:id>GAZ:00066383</oboInOwl:id>
        <rdfs:label>Nabaroh Region</rdfs:label>
    </owl:NamedIndividual>
    


    <!-- http://purl.obolibrary.org/obo/GAZ_00066384 -->

    <owl:NamedIndividual rdf:about="http://purl.obolibrary.org/obo/GAZ_00066384">
        <obo:RO_0001025 rdf:resource="http://purl.obolibrary.org/obo/GAZ_00000648"/>
        <obo:IAO_0000115>An administrative region (markaz) of Faiyum Governorate.</obo:IAO_0000115>
        <oboInOwl:hasOBONamespace>GAZ</oboInOwl:hasOBONamespace>
        <oboInOwl:id>GAZ:00066384</oboInOwl:id>
        <rdfs:label>Alfayom Region</rdfs:label>
    </owl:NamedIndividual>
    


    <!-- http://purl.obolibrary.org/obo/GAZ_00066385 -->

    <owl:NamedIndividual rdf:about="http://purl.obolibrary.org/obo/GAZ_00066385">
        <obo:RO_0001025 rdf:resource="http://purl.obolibrary.org/obo/GAZ_00000648"/>
        <obo:IAO_0000115>A distinctive region with character between the main Nile Valley and other desert oases. It is a depression in the desert immediately to the west of the Nile south of Cairo. Much of its floor is fields watered by a channel of the Nile, the Bahr Yussef, as it drains into a desert depression to the west of the Nile Valley. The Bahr Yussef veers west through a narrow neck of land north of Ihnasya, between the archaeological sites of El-Lahun and Gurob near Hawara; it then branches out, providing rich agricultural land in the Faiyum basin, draining into the large saltwater Lake Moeris (Birket Qarun). Lake Moeris was freshwater in prehistory but is today a saltwater lake.</obo:IAO_0000115>
        <oboInOwl:hasOBONamespace>GAZ</oboInOwl:hasOBONamespace>
        <oboInOwl:id>GAZ:00066385</oboInOwl:id>
        <rdfs:label>Faiyum Oasis</rdfs:label>
    </owl:NamedIndividual>
    


    <!-- http://purl.obolibrary.org/obo/GAZ_00066386 -->

    <owl:NamedIndividual rdf:about="http://purl.obolibrary.org/obo/GAZ_00066386">
        <obo:RO_0001025 rdf:resource="http://purl.obolibrary.org/obo/GAZ_00000658"/>
        <obo:IAO_0000115>An administrative region (markaz) of Gharbia Governorate.</obo:IAO_0000115>
        <oboInOwl:hasOBONamespace>GAZ</oboInOwl:hasOBONamespace>
        <oboInOwl:id>GAZ:00066386</oboInOwl:id>
        <rdfs:label>Elmahlah Alkobra Region</rdfs:label>
    </owl:NamedIndividual>
    


    <!-- http://purl.obolibrary.org/obo/GAZ_00066387 -->

    <owl:NamedIndividual rdf:about="http://purl.obolibrary.org/obo/GAZ_00066387">
        <obo:RO_0001025 rdf:resource="http://purl.obolibrary.org/obo/GAZ_00000664"/>
        <obo:IAO_0000115>An administrative region (markaz) of Ismalia Governorate.</obo:IAO_0000115>
        <oboInOwl:hasOBONamespace>GAZ</oboInOwl:hasOBONamespace>
        <oboInOwl:id>GAZ:00066387</oboInOwl:id>
        <rdfs:label>Fayed Region</rdfs:label>
    </owl:NamedIndividual>
    


    <!-- http://purl.obolibrary.org/obo/GAZ_00066389 -->

    <owl:NamedIndividual rdf:about="http://purl.obolibrary.org/obo/GAZ_00066389">
        <obo:RO_0001025 rdf:resource="http://purl.obolibrary.org/obo/GAZ_00000649"/>
        <obo:IAO_0000115>An administrative region (kism) of Giza Governorate.</obo:IAO_0000115>
        <oboInOwl:hasOBONamespace>GAZ</oboInOwl:hasOBONamespace>
        <oboInOwl:id>GAZ:00066389</oboInOwl:id>
        <rdfs:label>Kism Bulaq ad Dakrur</rdfs:label>
    </owl:NamedIndividual>
    


    <!-- http://purl.obolibrary.org/obo/GAZ_00066392 -->

    <owl:NamedIndividual rdf:about="http://purl.obolibrary.org/obo/GAZ_00066392">
        <obo:RO_0001025 rdf:resource="http://purl.obolibrary.org/obo/GAZ_00000649"/>
        <obo:IAO_0000115>An administrative region (kism) of Giza Governorate.</obo:IAO_0000115>
        <oboInOwl:hasOBONamespace>GAZ</oboInOwl:hasOBONamespace>
        <oboInOwl:id>GAZ:00066392</oboInOwl:id>
        <rdfs:label>Kism Al Hawamidiyah</rdfs:label>
    </owl:NamedIndividual>
    


    <!-- http://purl.obolibrary.org/obo/GAZ_00066396 -->

    <owl:NamedIndividual rdf:about="http://purl.obolibrary.org/obo/GAZ_00066396">
        <obo:RO_0001025 rdf:resource="http://purl.obolibrary.org/obo/GAZ_00000649"/>
        <obo:IAO_0000115>An oasis in Egypt. It is approximately 300 km away from Cairo and the least technologically advanced Oasis in the country. Located in Giza Governorate.</obo:IAO_0000115>
        <oboInOwl:hasOBONamespace>GAZ</oboInOwl:hasOBONamespace>
        <oboInOwl:id>GAZ:00066396</oboInOwl:id>
        <rdfs:label>Bahariya Oasis</rdfs:label>
    </owl:NamedIndividual>
    


    <!-- http://purl.obolibrary.org/obo/GAZ_00066397 -->

    <owl:NamedIndividual rdf:about="http://purl.obolibrary.org/obo/GAZ_00066397">
        <obo:RO_0001025 rdf:resource="http://purl.obolibrary.org/obo/GAZ_00000664"/>
        <obo:IAO_0000115>An administrative region (markaz) of Ismalia Governorate.</obo:IAO_0000115>
        <oboInOwl:hasOBONamespace>GAZ</oboInOwl:hasOBONamespace>
        <oboInOwl:id>GAZ:00066397</oboInOwl:id>
        <rdfs:label>Ismailia Region</rdfs:label>
    </owl:NamedIndividual>
    


    <!-- http://purl.obolibrary.org/obo/GAZ_00066398 -->

    <owl:NamedIndividual rdf:about="http://purl.obolibrary.org/obo/GAZ_00066398">
        <obo:RO_0001025 rdf:resource="http://purl.obolibrary.org/obo/GAZ_00000667"/>
        <obo:IAO_0000115>An administrative region (markaz) of Matruh Governorate.</obo:IAO_0000115>
        <oboInOwl:hasOBONamespace>GAZ</oboInOwl:hasOBONamespace>
        <oboInOwl:id>GAZ:00066398</oboInOwl:id>
        <rdfs:label>Sewa Region</rdfs:label>
    </owl:NamedIndividual>
    


    <!-- http://purl.obolibrary.org/obo/GAZ_00066399 -->

    <owl:NamedIndividual rdf:about="http://purl.obolibrary.org/obo/GAZ_00066399">
        <obo:RO_0001025 rdf:resource="http://purl.obolibrary.org/obo/GAZ_00089781"/>
        <obo:IAO_0000115>A saline lake in the N of Kafr el-Sheikh Governorate.</obo:IAO_0000115>
        <oboInOwl:hasOBONamespace>GAZ</oboInOwl:hasOBONamespace>
        <oboInOwl:id>GAZ:00066399</oboInOwl:id>
        <rdfs:label>Buhayrat al-Burullus</rdfs:label>
    </owl:NamedIndividual>
    


    <!-- http://purl.obolibrary.org/obo/GAZ_00066400 -->

    <owl:NamedIndividual rdf:about="http://purl.obolibrary.org/obo/GAZ_00066400"/>
    


    <!-- http://purl.obolibrary.org/obo/GAZ_00066402 -->

    <owl:NamedIndividual rdf:about="http://purl.obolibrary.org/obo/GAZ_00066402">
        <obo:RO_0001025 rdf:resource="http://purl.obolibrary.org/obo/GAZ_00066400"/>
        <obo:IAO_0000115>An administrative region (markaz) of Luxor Governorate.</obo:IAO_0000115>
        <oboInOwl:hasOBONamespace>GAZ</oboInOwl:hasOBONamespace>
        <oboInOwl:id>GAZ:00066402</oboInOwl:id>
        <rdfs:label>Luxor Region</rdfs:label>
    </owl:NamedIndividual>
    


    <!-- http://purl.obolibrary.org/obo/GAZ_00066405 -->

    <owl:NamedIndividual rdf:about="http://purl.obolibrary.org/obo/GAZ_00066405">
        <obo:RO_0001025 rdf:resource="http://purl.obolibrary.org/obo/GAZ_00000661"/>
        <obo:IAO_0000115>An administrative region (markaz) of Qalyubia Governorate.</obo:IAO_0000115>
        <oboInOwl:hasOBONamespace>GAZ</oboInOwl:hasOBONamespace>
        <oboInOwl:id>GAZ:00066405</oboInOwl:id>
        <rdfs:label>Kafr Shokr Region</rdfs:label>
    </owl:NamedIndividual>
    


    <!-- http://purl.obolibrary.org/obo/GAZ_00066406 -->

    <owl:NamedIndividual rdf:about="http://purl.obolibrary.org/obo/GAZ_00066406">
        <obo:RO_0001025 rdf:resource="http://purl.obolibrary.org/obo/GAZ_00000668"/>
        <obo:IAO_0000115>An administrative region (markaz) of New Valley Governorate.</obo:IAO_0000115>
        <oboInOwl:hasOBONamespace>GAZ</oboInOwl:hasOBONamespace>
        <oboInOwl:id>GAZ:00066406</oboInOwl:id>
        <rdfs:label>Alfrafrah Region</rdfs:label>
    </owl:NamedIndividual>
    


    <!-- http://purl.obolibrary.org/obo/GAZ_00066407 -->

    <owl:NamedIndividual rdf:about="http://purl.obolibrary.org/obo/GAZ_00066407">
        <obo:RO_0001025 rdf:resource="http://purl.obolibrary.org/obo/GAZ_00000668"/>
        <obo:IAO_0000115>An administrative region (markaz) of New Valley Governorate.</obo:IAO_0000115>
        <oboInOwl:hasOBONamespace>GAZ</oboInOwl:hasOBONamespace>
        <oboInOwl:id>GAZ:00066407</oboInOwl:id>
        <rdfs:label>Aldakhlah Region</rdfs:label>
    </owl:NamedIndividual>
    


    <!-- http://purl.obolibrary.org/obo/GAZ_00066408 -->

    <owl:NamedIndividual rdf:about="http://purl.obolibrary.org/obo/GAZ_00066408">
        <obo:RO_0001025 rdf:resource="http://purl.obolibrary.org/obo/GAZ_00000668"/>
        <obo:IAO_0000115>An administrative region (markaz) of New Valley Governorate.</obo:IAO_0000115>
        <oboInOwl:hasOBONamespace>GAZ</oboInOwl:hasOBONamespace>
        <oboInOwl:id>GAZ:00066408</oboInOwl:id>
        <rdfs:label>Alkhargah Region</rdfs:label>
    </owl:NamedIndividual>
    


    <!-- http://purl.obolibrary.org/obo/GAZ_00066409 -->

    <owl:NamedIndividual rdf:about="http://purl.obolibrary.org/obo/GAZ_00066409">
        <obo:RO_0001025 rdf:resource="http://purl.obolibrary.org/obo/GAZ_00248009"/>
        <obo:IAO_0000115>An oasis in Egypt, located between the Qattara Depression and the Egyptian Sand Sea in the Libyan Desert, nearly 50 km east of the Libyan border, and 560 km from Cairo.</obo:IAO_0000115>
        <oboInOwl:hasOBONamespace>GAZ</oboInOwl:hasOBONamespace>
        <oboInOwl:id>GAZ:00066409</oboInOwl:id>
        <rdfs:label>Siwa Oasis</rdfs:label>
    </owl:NamedIndividual>
    


    <!-- http://purl.obolibrary.org/obo/GAZ_00066410 -->

    <owl:NamedIndividual rdf:about="http://purl.obolibrary.org/obo/GAZ_00066410">
        <obo:RO_0001025 rdf:resource="http://purl.obolibrary.org/obo/GAZ_00051197"/>
        <obo:IAO_0000115>A desert located 45 km north of Farafra. The desert has a white, cream color and has massive chalk rock formations that have been created as a result of occasional sandstorms in the area.</obo:IAO_0000115>
        <oboInOwl:hasOBONamespace>GAZ</oboInOwl:hasOBONamespace>
        <oboInOwl:id>GAZ:00066410</oboInOwl:id>
        <rdfs:label>Sahara el Beyda</rdfs:label>
    </owl:NamedIndividual>
    


    <!-- http://purl.obolibrary.org/obo/GAZ_00066411 -->

    <owl:NamedIndividual rdf:about="http://purl.obolibrary.org/obo/GAZ_00066411">
        <obo:RO_0001025 rdf:resource="http://purl.obolibrary.org/obo/GAZ_00000665"/>
        <oboInOwl:hasOBONamespace>GAZ</oboInOwl:hasOBONamespace>
        <oboInOwl:id>GAZ:00066411</oboInOwl:id>
        <rdfs:label>Port Said District</rdfs:label>
    </owl:NamedIndividual>
    


    <!-- http://purl.obolibrary.org/obo/GAZ_00066412 -->

    <owl:NamedIndividual rdf:about="http://purl.obolibrary.org/obo/GAZ_00066412">
        <obo:RO_0001025 rdf:resource="http://purl.obolibrary.org/obo/GAZ_00000661"/>
        <obo:IAO_0000115>An administrative region (markaz) of Qalyubia Governorate.</obo:IAO_0000115>
        <oboInOwl:hasOBONamespace>GAZ</oboInOwl:hasOBONamespace>
        <oboInOwl:id>GAZ:00066412</oboInOwl:id>
        <rdfs:label>Alkanater Alkhyriah Region</rdfs:label>
    </owl:NamedIndividual>
    


    <!-- http://purl.obolibrary.org/obo/GAZ_00066413 -->

    <owl:NamedIndividual rdf:about="http://purl.obolibrary.org/obo/GAZ_00066413">
        <obo:RO_0001025 rdf:resource="http://purl.obolibrary.org/obo/GAZ_00000654"/>
        <obo:IAO_0000115>An administrative region (kism) of Red Sea Governorate.</obo:IAO_0000115>
        <oboInOwl:hasOBONamespace>GAZ</oboInOwl:hasOBONamespace>
        <oboInOwl:id>GAZ:00066413</oboInOwl:id>
        <rdfs:label>Kism Safajah</rdfs:label>
    </owl:NamedIndividual>
    


    <!-- http://purl.obolibrary.org/obo/GAZ_00066414 -->

    <owl:NamedIndividual rdf:about="http://purl.obolibrary.org/obo/GAZ_00066414">
        <obo:RO_0001025 rdf:resource="http://purl.obolibrary.org/obo/GAZ_00000654"/>
        <obo:IAO_0000115>An administrative region (kism) of Red Sea Governorate.</obo:IAO_0000115>
        <oboInOwl:hasOBONamespace>GAZ</oboInOwl:hasOBONamespace>
        <oboInOwl:id>GAZ:00066414</oboInOwl:id>
        <rdfs:label>Kism Ra&apos;s Gharib</rdfs:label>
    </owl:NamedIndividual>
    


    <!-- http://purl.obolibrary.org/obo/GAZ_00066415 -->

    <owl:NamedIndividual rdf:about="http://purl.obolibrary.org/obo/GAZ_00066415">
        <obo:RO_0001025 rdf:resource="http://purl.obolibrary.org/obo/GAZ_00000654"/>
        <obo:IAO_0000115>An administrative region (kism) of Red Sea Governorate.</obo:IAO_0000115>
        <oboInOwl:hasOBONamespace>GAZ</oboInOwl:hasOBONamespace>
        <oboInOwl:id>GAZ:00066415</oboInOwl:id>
        <rdfs:label>Kism Al Ghardaqah</rdfs:label>
    </owl:NamedIndividual>
    


    <!-- http://purl.obolibrary.org/obo/GAZ_00066416 -->

    <owl:NamedIndividual rdf:about="http://purl.obolibrary.org/obo/GAZ_00066416">
        <obo:RO_0001025 rdf:resource="http://purl.obolibrary.org/obo/GAZ_00000654"/>
        <obo:IAO_0000115>An administrative region (kism) of Red Sea Governorate.</obo:IAO_0000115>
        <oboInOwl:hasOBONamespace>GAZ</oboInOwl:hasOBONamespace>
        <oboInOwl:id>GAZ:00066416</oboInOwl:id>
        <rdfs:label>Kism Al Qusayr</rdfs:label>
    </owl:NamedIndividual>
    


    <!-- http://purl.obolibrary.org/obo/GAZ_00066417 -->

    <owl:NamedIndividual rdf:about="http://purl.obolibrary.org/obo/GAZ_00066417">
        <obo:RO_0001025 rdf:resource="http://purl.obolibrary.org/obo/GAZ_00000662"/>
        <obo:IAO_0000115>An administrative region (markaz) of Sharqia Governorate.</obo:IAO_0000115>
        <oboInOwl:hasOBONamespace>GAZ</oboInOwl:hasOBONamespace>
        <oboInOwl:id>GAZ:00066417</oboInOwl:id>
        <rdfs:label>Mashtoul Alsouk Region</rdfs:label>
    </owl:NamedIndividual>
    


    <!-- http://purl.obolibrary.org/obo/GAZ_00066418 -->

    <owl:NamedIndividual rdf:about="http://purl.obolibrary.org/obo/GAZ_00066418">
        <obo:RO_0001025 rdf:resource="http://purl.obolibrary.org/obo/GAZ_00000669"/>
        <obo:IAO_0000115>An administrative region (markaz) of North Sinai Governorate.</obo:IAO_0000115>
        <oboInOwl:hasOBONamespace>GAZ</oboInOwl:hasOBONamespace>
        <oboInOwl:id>GAZ:00066418</oboInOwl:id>
        <rdfs:label>Alsheikh Zwayed Region</rdfs:label>
    </owl:NamedIndividual>
    


    <!-- http://purl.obolibrary.org/obo/GAZ_00066420 -->

    <owl:NamedIndividual rdf:about="http://purl.obolibrary.org/obo/GAZ_00066420">
        <obo:RO_0001025 rdf:resource="http://purl.obolibrary.org/obo/GAZ_00000666"/>
        <obo:IAO_0000115>An administrative region (kism) of Suez Governorate.</obo:IAO_0000115>
        <oboInOwl:hasOBONamespace>GAZ</oboInOwl:hasOBONamespace>
        <oboInOwl:id>GAZ:00066420</oboInOwl:id>
        <rdfs:label>Kism As Suways</rdfs:label>
    </owl:NamedIndividual>
    


    <!-- http://purl.obolibrary.org/obo/GAZ_00066421 -->

    <owl:NamedIndividual rdf:about="http://purl.obolibrary.org/obo/GAZ_00066421">
        <obo:RO_0001025 rdf:resource="http://purl.obolibrary.org/obo/GAZ_00000666"/>
        <obo:IAO_0000115>An administrative region (kism) of Suez Governorate.</obo:IAO_0000115>
        <oboInOwl:hasOBONamespace>GAZ</oboInOwl:hasOBONamespace>
        <oboInOwl:id>GAZ:00066421</oboInOwl:id>
        <rdfs:label>Kism Al Jana&apos;in</rdfs:label>
    </owl:NamedIndividual>
    


    <!-- http://purl.obolibrary.org/obo/GAZ_00066422 -->

    <owl:NamedIndividual rdf:about="http://purl.obolibrary.org/obo/GAZ_00066422">
        <obo:RO_0001025 rdf:resource="http://purl.obolibrary.org/obo/GAZ_00000666"/>
        <obo:IAO_0000115>An administrative region (kism) of Suez Governorate.</obo:IAO_0000115>
        <oboInOwl:hasOBONamespace>GAZ</oboInOwl:hasOBONamespace>
        <oboInOwl:id>GAZ:00066422</oboInOwl:id>
        <rdfs:label>Kism &apos;Ataqah</rdfs:label>
    </owl:NamedIndividual>
    


    <!-- http://purl.obolibrary.org/obo/GAZ_00066423 -->

    <owl:NamedIndividual rdf:about="http://purl.obolibrary.org/obo/GAZ_00066423">
        <obo:RO_0001025 rdf:resource="http://purl.obolibrary.org/obo/GAZ_00000669"/>
        <oboInOwl:hasOBONamespace>GAZ</oboInOwl:hasOBONamespace>
        <oboInOwl:id>GAZ:00066423</oboInOwl:id>
        <rdfs:label>Alaresh Region</rdfs:label>
    </owl:NamedIndividual>
    


    <!-- http://purl.obolibrary.org/obo/GAZ_00066424 -->

    <owl:NamedIndividual rdf:about="http://purl.obolibrary.org/obo/GAZ_00066424">
        <obo:RO_0001025 rdf:resource="http://purl.obolibrary.org/obo/GAZ_00000669"/>
        <obo:IAO_0000115>An administrative region (markaz) of North Sinai Governorate.</obo:IAO_0000115>
        <oboInOwl:hasOBONamespace>GAZ</oboInOwl:hasOBONamespace>
        <oboInOwl:id>GAZ:00066424</oboInOwl:id>
        <rdfs:label>Nekhel Region</rdfs:label>
    </owl:NamedIndividual>
    


    <!-- http://purl.obolibrary.org/obo/GAZ_00066425 -->

    <owl:NamedIndividual rdf:about="http://purl.obolibrary.org/obo/GAZ_00066425">
        <obo:RO_0001025 rdf:resource="http://purl.obolibrary.org/obo/GAZ_00000669"/>
        <obo:IAO_0000115>An administrative region (markaz) of North Sinai Governorate.</obo:IAO_0000115>
        <oboInOwl:hasOBONamespace>GAZ</oboInOwl:hasOBONamespace>
        <oboInOwl:id>GAZ:00066425</oboInOwl:id>
        <rdfs:label>Alhasanah Region</rdfs:label>
    </owl:NamedIndividual>
    


    <!-- http://purl.obolibrary.org/obo/GAZ_00066426 -->

    <owl:NamedIndividual rdf:about="http://purl.obolibrary.org/obo/GAZ_00066426">
        <obo:RO_0001025 rdf:resource="http://purl.obolibrary.org/obo/GAZ_00000669"/>
        <obo:IAO_0000115>An administrative region (markaz) of North Sinai Governorate.</obo:IAO_0000115>
        <oboInOwl:hasOBONamespace>GAZ</oboInOwl:hasOBONamespace>
        <oboInOwl:id>GAZ:00066426</oboInOwl:id>
        <rdfs:label>Rafah Region</rdfs:label>
    </owl:NamedIndividual>
    


    <!-- http://purl.obolibrary.org/obo/GAZ_00066427 -->

    <owl:NamedIndividual rdf:about="http://purl.obolibrary.org/obo/GAZ_00066427">
        <obo:RO_0001025 rdf:resource="http://purl.obolibrary.org/obo/GAZ_00000669"/>
        <obo:IAO_0000115>An administrative region (kism) of North Sinai Governorate.</obo:IAO_0000115>
        <oboInOwl:hasOBONamespace>GAZ</oboInOwl:hasOBONamespace>
        <oboInOwl:id>GAZ:00066427</oboInOwl:id>
        <rdfs:label>Kism Bi&apos;r al&apos;Abd</rdfs:label>
    </owl:NamedIndividual>
    


    <!-- http://purl.obolibrary.org/obo/GAZ_00066428 -->

    <owl:NamedIndividual rdf:about="http://purl.obolibrary.org/obo/GAZ_00066428">
        <obo:RO_0001025 rdf:resource="http://purl.obolibrary.org/obo/GAZ_00051197"/>
        <obo:IAO_0000115>An oasis with a large lake located in the municipality Sabha in the Libyan Sahara. The lake is saline.</obo:IAO_0000115>
        <oboInOwl:hasOBONamespace>GAZ</oboInOwl:hasOBONamespace>
        <oboInOwl:id>GAZ:00066428</oboInOwl:id>
        <rdfs:label>Gaberoun Oasis</rdfs:label>
    </owl:NamedIndividual>
    


    <!-- http://purl.obolibrary.org/obo/GAZ_00066429 -->

    <owl:NamedIndividual rdf:about="http://purl.obolibrary.org/obo/GAZ_00066429">
        <obo:RO_0001025 rdf:resource="http://purl.obolibrary.org/obo/GAZ_00051197"/>
        <obo:IAO_0000115>An erg.</obo:IAO_0000115>
        <oboInOwl:hasOBONamespace>GAZ</oboInOwl:hasOBONamespace>
        <oboInOwl:id>GAZ:00066429</oboInOwl:id>
        <rdfs:label>Ramlat al Dauada</rdfs:label>
    </owl:NamedIndividual>
    


    <!-- http://purl.obolibrary.org/obo/GAZ_00066430 -->

    <owl:NamedIndividual rdf:about="http://purl.obolibrary.org/obo/GAZ_00066430">
        <obo:RO_0001025 rdf:resource="http://purl.obolibrary.org/obo/GAZ_00066429"/>
        <obo:IAO_0000115>A lake in the Ramlat al Dauada erg.</obo:IAO_0000115>
        <oboInOwl:hasOBONamespace>GAZ</oboInOwl:hasOBONamespace>
        <oboInOwl:id>GAZ:00066430</oboInOwl:id>
        <rdfs:label>Mafo Lake</rdfs:label>
    </owl:NamedIndividual>
    


    <!-- http://purl.obolibrary.org/obo/GAZ_00066431 -->

    <owl:NamedIndividual rdf:about="http://purl.obolibrary.org/obo/GAZ_00066431">
        <obo:RO_0001025 rdf:resource="http://purl.obolibrary.org/obo/GAZ_00051197"/>
        <obo:IAO_0000115>An oasis in Southeastern Libya.</obo:IAO_0000115>
        <oboInOwl:hasOBONamespace>GAZ</oboInOwl:hasOBONamespace>
        <oboInOwl:id>GAZ:00066431</oboInOwl:id>
        <rdfs:label>Kufra Oasis</rdfs:label>
    </owl:NamedIndividual>
    


    <!-- http://purl.obolibrary.org/obo/GAZ_00066446 -->

    <owl:NamedIndividual rdf:about="http://purl.obolibrary.org/obo/GAZ_00066446">
        <obo:RO_0001025 rdf:resource="http://purl.obolibrary.org/obo/GAZ_00000667"/>
        <obo:IAO_0000115>An administrative region (markaz) of Matruh Governorate.</obo:IAO_0000115>
        <oboInOwl:hasOBONamespace>GAZ</oboInOwl:hasOBONamespace>
        <oboInOwl:id>GAZ:00066446</oboInOwl:id>
        <rdfs:label>Seidy Barrany Region</rdfs:label>
    </owl:NamedIndividual>
    


    <!-- http://purl.obolibrary.org/obo/GAZ_00066447 -->

    <owl:NamedIndividual rdf:about="http://purl.obolibrary.org/obo/GAZ_00066447">
        <obo:RO_0001025 rdf:resource="http://purl.obolibrary.org/obo/GAZ_00000667"/>
        <obo:IAO_0000115>An administrative region (markaz) of Matruh Governorate.</obo:IAO_0000115>
        <oboInOwl:hasOBONamespace>GAZ</oboInOwl:hasOBONamespace>
        <oboInOwl:id>GAZ:00066447</oboInOwl:id>
        <rdfs:label>Aldabaa Region</rdfs:label>
    </owl:NamedIndividual>
    


    <!-- http://purl.obolibrary.org/obo/GAZ_00066448 -->

    <owl:NamedIndividual rdf:about="http://purl.obolibrary.org/obo/GAZ_00066448">
        <obo:RO_0001025 rdf:resource="http://purl.obolibrary.org/obo/GAZ_00241990"/>
        <obo:IAO_0000115>A populated place. A city 240 km west of Alexandria, along the shore of the Mediterranean Sea.</obo:IAO_0000115>
        <oboInOwl:hasOBONamespace>GAZ</oboInOwl:hasOBONamespace>
        <oboInOwl:id>GAZ:00066448</oboInOwl:id>
        <rdfs:label>Mersa Matruh</rdfs:label>
    </owl:NamedIndividual>
    


    <!-- http://purl.obolibrary.org/obo/GAZ_00066449 -->

    <owl:NamedIndividual rdf:about="http://purl.obolibrary.org/obo/GAZ_00066449">
        <obo:RO_0001025 rdf:resource="http://purl.obolibrary.org/obo/GAZ_00000667"/>
        <obo:IAO_0000115>An administrative region (markaz) of Matruh Governorate.</obo:IAO_0000115>
        <oboInOwl:hasOBONamespace>GAZ</oboInOwl:hasOBONamespace>
        <oboInOwl:id>GAZ:00066449</oboInOwl:id>
        <rdfs:label>Alhammam Region</rdfs:label>
    </owl:NamedIndividual>
    


    <!-- http://purl.obolibrary.org/obo/GAZ_00066450 -->

    <owl:NamedIndividual rdf:about="http://purl.obolibrary.org/obo/GAZ_00066450">
        <obo:RO_0001025 rdf:resource="http://purl.obolibrary.org/obo/GAZ_00000667"/>
        <obo:IAO_0000115>An administrative region (markaz) of Matruh Governorate.</obo:IAO_0000115>
        <oboInOwl:hasOBONamespace>GAZ</oboInOwl:hasOBONamespace>
        <oboInOwl:id>GAZ:00066450</oboInOwl:id>
        <rdfs:label>Alnagela Region</rdfs:label>
    </owl:NamedIndividual>
    


    <!-- http://purl.obolibrary.org/obo/GAZ_00066451 -->

    <owl:NamedIndividual rdf:about="http://purl.obolibrary.org/obo/GAZ_00066451">
        <obo:RO_0001025 rdf:resource="http://purl.obolibrary.org/obo/GAZ_00000667"/>
        <obo:IAO_0000115>An administrative region (markaz) of Matruh Governorate.</obo:IAO_0000115>
        <oboInOwl:hasOBONamespace>GAZ</oboInOwl:hasOBONamespace>
        <oboInOwl:id>GAZ:00066451</oboInOwl:id>
        <rdfs:label>Alalameen Region</rdfs:label>
    </owl:NamedIndividual>
    


    <!-- http://purl.obolibrary.org/obo/GAZ_00066452 -->

    <owl:NamedIndividual rdf:about="http://purl.obolibrary.org/obo/GAZ_00066452">
        <obo:RO_0001025 rdf:resource="http://purl.obolibrary.org/obo/GAZ_00000664"/>
        <obo:IAO_0000115>An administrative region (kism) of Ismalia Governorate.</obo:IAO_0000115>
        <oboInOwl:hasOBONamespace>GAZ</oboInOwl:hasOBONamespace>
        <oboInOwl:id>GAZ:00066452</oboInOwl:id>
        <rdfs:label>Kism Al Qantarah ash Sharqiyah</rdfs:label>
    </owl:NamedIndividual>
    


    <!-- http://purl.obolibrary.org/obo/GAZ_00066453 -->

    <owl:NamedIndividual rdf:about="http://purl.obolibrary.org/obo/GAZ_00066453">
        <obo:RO_0001025 rdf:resource="http://purl.obolibrary.org/obo/GAZ_00000664"/>
        <obo:IAO_0000115>An administrative region (markaz) of Ismalia Governorate.</obo:IAO_0000115>
        <oboInOwl:hasOBONamespace>GAZ</oboInOwl:hasOBONamespace>
        <oboInOwl:id>GAZ:00066453</oboInOwl:id>
        <rdfs:label>Alkantara Gharb Region</rdfs:label>
    </owl:NamedIndividual>
    


    <!-- http://purl.obolibrary.org/obo/GAZ_00066454 -->

    <owl:NamedIndividual rdf:about="http://purl.obolibrary.org/obo/GAZ_00066454">
        <obo:RO_0001025 rdf:resource="http://purl.obolibrary.org/obo/GAZ_00000664"/>
        <obo:IAO_0000115>An administrative region (markaz) of Ismalia Governorate.</obo:IAO_0000115>
        <oboInOwl:hasOBONamespace>GAZ</oboInOwl:hasOBONamespace>
        <oboInOwl:id>GAZ:00066454</oboInOwl:id>
        <rdfs:label>Eltal Elkabeer Region</rdfs:label>
    </owl:NamedIndividual>
    


    <!-- http://purl.obolibrary.org/obo/GAZ_00066455 -->

    <owl:NamedIndividual rdf:about="http://purl.obolibrary.org/obo/GAZ_00066455">
        <obo:RO_0001025 rdf:resource="http://purl.obolibrary.org/obo/GAZ_00000658"/>
        <obo:IAO_0000115>An administrative region (markaz) of Gharbia Governorate.</obo:IAO_0000115>
        <oboInOwl:hasOBONamespace>GAZ</oboInOwl:hasOBONamespace>
        <oboInOwl:id>GAZ:00066455</oboInOwl:id>
        <rdfs:label>Samnoud Region</rdfs:label>
    </owl:NamedIndividual>
    


    <!-- http://purl.obolibrary.org/obo/GAZ_00066456 -->

    <owl:NamedIndividual rdf:about="http://purl.obolibrary.org/obo/GAZ_00066456">
        <obo:RO_0001025 rdf:resource="http://purl.obolibrary.org/obo/GAZ_00000658"/>
        <obo:IAO_0000115>An administrative region (markaz) of Gharbia Governorate.</obo:IAO_0000115>
        <oboInOwl:hasOBONamespace>GAZ</oboInOwl:hasOBONamespace>
        <oboInOwl:id>GAZ:00066456</oboInOwl:id>
        <rdfs:label>Zefta Region</rdfs:label>
    </owl:NamedIndividual>
    


    <!-- http://purl.obolibrary.org/obo/GAZ_00066457 -->

    <owl:NamedIndividual rdf:about="http://purl.obolibrary.org/obo/GAZ_00066457">
        <obo:RO_0001025 rdf:resource="http://purl.obolibrary.org/obo/GAZ_00000658"/>
        <obo:IAO_0000115>An administrative region (markaz) of Gharbia Governorate.</obo:IAO_0000115>
        <oboInOwl:hasOBONamespace>GAZ</oboInOwl:hasOBONamespace>
        <oboInOwl:id>GAZ:00066457</oboInOwl:id>
        <rdfs:label>Elsanta Region</rdfs:label>
    </owl:NamedIndividual>
    


    <!-- http://purl.obolibrary.org/obo/GAZ_00066458 -->

    <owl:NamedIndividual rdf:about="http://purl.obolibrary.org/obo/GAZ_00066458">
        <obo:RO_0001025 rdf:resource="http://purl.obolibrary.org/obo/GAZ_00000658"/>
        <obo:IAO_0000115>An administrative region (markaz) of Gharbia Governorate.</obo:IAO_0000115>
        <oboInOwl:hasOBONamespace>GAZ</oboInOwl:hasOBONamespace>
        <oboInOwl:id>GAZ:00066458</oboInOwl:id>
        <rdfs:label>Basyoun Region</rdfs:label>
    </owl:NamedIndividual>
    


    <!-- http://purl.obolibrary.org/obo/GAZ_00066459 -->

    <owl:NamedIndividual rdf:about="http://purl.obolibrary.org/obo/GAZ_00066459">
        <obo:RO_0001025 rdf:resource="http://purl.obolibrary.org/obo/GAZ_00000658"/>
        <obo:IAO_0000115>An administrative region (markaz) of Gharbia Governorate.</obo:IAO_0000115>
        <oboInOwl:hasOBONamespace>GAZ</oboInOwl:hasOBONamespace>
        <oboInOwl:id>GAZ:00066459</oboInOwl:id>
        <rdfs:label>Tanta Region</rdfs:label>
    </owl:NamedIndividual>
    


    <!-- http://purl.obolibrary.org/obo/GAZ_00066460 -->

    <owl:NamedIndividual rdf:about="http://purl.obolibrary.org/obo/GAZ_00066460">
        <obo:RO_0001025 rdf:resource="http://purl.obolibrary.org/obo/GAZ_00000658"/>
        <obo:IAO_0000115>An administrative region (markaz) of Gharbia Governorate.</obo:IAO_0000115>
        <oboInOwl:hasOBONamespace>GAZ</oboInOwl:hasOBONamespace>
        <oboInOwl:id>GAZ:00066460</oboInOwl:id>
        <rdfs:label>Qoutor Region</rdfs:label>
    </owl:NamedIndividual>
    


    <!-- http://purl.obolibrary.org/obo/GAZ_00066461 -->

    <owl:NamedIndividual rdf:about="http://purl.obolibrary.org/obo/GAZ_00066461">
        <obo:RO_0001025 rdf:resource="http://purl.obolibrary.org/obo/GAZ_00000658"/>
        <obo:IAO_0000115>An administrative region (markaz) of Gharbia Governorate.</obo:IAO_0000115>
        <oboInOwl:hasOBONamespace>GAZ</oboInOwl:hasOBONamespace>
        <oboInOwl:id>GAZ:00066461</oboInOwl:id>
        <rdfs:label>Kafr Elzayat Region</rdfs:label>
    </owl:NamedIndividual>
    


    <!-- http://purl.obolibrary.org/obo/GAZ_00066462 -->

    <owl:NamedIndividual rdf:about="http://purl.obolibrary.org/obo/GAZ_00066462">
        <obo:RO_0001025 rdf:resource="http://purl.obolibrary.org/obo/GAZ_00000648"/>
        <obo:IAO_0000115>An administrative region (markaz) of Faiyum Governorate.</obo:IAO_0000115>
        <oboInOwl:hasOBONamespace>GAZ</oboInOwl:hasOBONamespace>
        <oboInOwl:id>GAZ:00066462</oboInOwl:id>
        <rdfs:label>Sennoris Region</rdfs:label>
    </owl:NamedIndividual>
    


    <!-- http://purl.obolibrary.org/obo/GAZ_00066463 -->

    <owl:NamedIndividual rdf:about="http://purl.obolibrary.org/obo/GAZ_00066463">
        <obo:RO_0001025 rdf:resource="http://purl.obolibrary.org/obo/GAZ_00000648"/>
        <obo:IAO_0000115>An administrative region (markaz) of Faiyum Governorate.</obo:IAO_0000115>
        <oboInOwl:hasOBONamespace>GAZ</oboInOwl:hasOBONamespace>
        <oboInOwl:id>GAZ:00066463</oboInOwl:id>
        <rdfs:label>Tamya Region</rdfs:label>
    </owl:NamedIndividual>
    


    <!-- http://purl.obolibrary.org/obo/GAZ_00066464 -->

    <owl:NamedIndividual rdf:about="http://purl.obolibrary.org/obo/GAZ_00066464">
        <obo:RO_0001025 rdf:resource="http://purl.obolibrary.org/obo/GAZ_00000648"/>
        <obo:IAO_0000115>An administrative region (markaz) of Faiyum Governorate.</obo:IAO_0000115>
        <oboInOwl:hasOBONamespace>GAZ</oboInOwl:hasOBONamespace>
        <oboInOwl:id>GAZ:00066464</oboInOwl:id>
        <rdfs:label>Etsa Region</rdfs:label>
    </owl:NamedIndividual>
    


    <!-- http://purl.obolibrary.org/obo/GAZ_00066465 -->

    <owl:NamedIndividual rdf:about="http://purl.obolibrary.org/obo/GAZ_00066465">
        <obo:RO_0001025 rdf:resource="http://purl.obolibrary.org/obo/GAZ_00000648"/>
        <obo:IAO_0000115>An administrative region (markaz) of Faiyum Governorate.</obo:IAO_0000115>
        <oboInOwl:hasOBONamespace>GAZ</oboInOwl:hasOBONamespace>
        <oboInOwl:id>GAZ:00066465</oboInOwl:id>
        <rdfs:label>Ebshaway Region</rdfs:label>
    </owl:NamedIndividual>
    


    <!-- http://purl.obolibrary.org/obo/GAZ_00066467 -->

    <owl:NamedIndividual rdf:about="http://purl.obolibrary.org/obo/GAZ_00066467">
        <obo:RO_0001025 rdf:resource="http://purl.obolibrary.org/obo/GAZ_00000647"/>
        <obo:IAO_0000115>An administrative region (markaz) of Beni Suef Governorate.</obo:IAO_0000115>
        <oboInOwl:hasOBONamespace>GAZ</oboInOwl:hasOBONamespace>
        <oboInOwl:id>GAZ:00066467</oboInOwl:id>
        <rdfs:label>Beba Region</rdfs:label>
    </owl:NamedIndividual>
    


    <!-- http://purl.obolibrary.org/obo/GAZ_00066468 -->

    <owl:NamedIndividual rdf:about="http://purl.obolibrary.org/obo/GAZ_00066468">
        <obo:RO_0001025 rdf:resource="http://purl.obolibrary.org/obo/GAZ_00000647"/>
        <obo:IAO_0000115>An administrative region (markaz) of Beni Suef Governorate.</obo:IAO_0000115>
        <oboInOwl:hasOBONamespace>GAZ</oboInOwl:hasOBONamespace>
        <oboInOwl:id>GAZ:00066468</oboInOwl:id>
        <rdfs:label>Naser Region</rdfs:label>
    </owl:NamedIndividual>
    


    <!-- http://purl.obolibrary.org/obo/GAZ_00066469 -->

    <owl:NamedIndividual rdf:about="http://purl.obolibrary.org/obo/GAZ_00066469">
        <obo:RO_0001025 rdf:resource="http://purl.obolibrary.org/obo/GAZ_00000647"/>
        <obo:IAO_0000115>An administrative region (markaz) of Beni Suef Governorate.</obo:IAO_0000115>
        <oboInOwl:hasOBONamespace>GAZ</oboInOwl:hasOBONamespace>
        <oboInOwl:id>GAZ:00066469</oboInOwl:id>
        <rdfs:label>Alwastah Region</rdfs:label>
    </owl:NamedIndividual>
    


    <!-- http://purl.obolibrary.org/obo/GAZ_00066470 -->

    <owl:NamedIndividual rdf:about="http://purl.obolibrary.org/obo/GAZ_00066470">
        <obo:RO_0001025 rdf:resource="http://purl.obolibrary.org/obo/GAZ_00000647"/>
        <obo:IAO_0000115>An administrative region (markaz) of Beni Suef Governorate.</obo:IAO_0000115>
        <oboInOwl:hasOBONamespace>GAZ</oboInOwl:hasOBONamespace>
        <oboInOwl:id>GAZ:00066470</oboInOwl:id>
        <rdfs:label>Ehnasia Region</rdfs:label>
    </owl:NamedIndividual>
    


    <!-- http://purl.obolibrary.org/obo/GAZ_00066472 -->

    <owl:NamedIndividual rdf:about="http://purl.obolibrary.org/obo/GAZ_00066472">
        <obo:RO_0001025 rdf:resource="http://purl.obolibrary.org/obo/GAZ_00000647"/>
        <obo:IAO_0000115>An administrative region (markaz) of Beni Suef Governorate.</obo:IAO_0000115>
        <oboInOwl:hasOBONamespace>GAZ</oboInOwl:hasOBONamespace>
        <oboInOwl:id>GAZ:00066472</oboInOwl:id>
        <rdfs:label>Alfashn Region</rdfs:label>
    </owl:NamedIndividual>
    


    <!-- http://purl.obolibrary.org/obo/GAZ_00066473 -->

    <owl:NamedIndividual rdf:about="http://purl.obolibrary.org/obo/GAZ_00066473">
        <obo:RO_0001025 rdf:resource="http://purl.obolibrary.org/obo/GAZ_00000655"/>
        <obo:IAO_0000115>An administrative region (markuz) of Beheira Governorate.</obo:IAO_0000115>
        <oboInOwl:hasOBONamespace>GAZ</oboInOwl:hasOBONamespace>
        <oboInOwl:id>GAZ:00066473</oboInOwl:id>
        <rdfs:label>Aldelengat Region</rdfs:label>
    </owl:NamedIndividual>
    


    <!-- http://purl.obolibrary.org/obo/GAZ_00066474 -->

    <owl:NamedIndividual rdf:about="http://purl.obolibrary.org/obo/GAZ_00066474">
        <obo:RO_0001025 rdf:resource="http://purl.obolibrary.org/obo/GAZ_00000655"/>
        <obo:IAO_0000115>An administrative region (markuz) of Beheira Governorate.</obo:IAO_0000115>
        <oboInOwl:hasOBONamespace>GAZ</oboInOwl:hasOBONamespace>
        <oboInOwl:id>GAZ:00066474</oboInOwl:id>
        <rdfs:label>Abou Elmatameer region</rdfs:label>
    </owl:NamedIndividual>
    


    <!-- http://purl.obolibrary.org/obo/GAZ_00066475 -->

    <owl:NamedIndividual rdf:about="http://purl.obolibrary.org/obo/GAZ_00066475">
        <obo:RO_0001025 rdf:resource="http://purl.obolibrary.org/obo/GAZ_00000655"/>
        <obo:IAO_0000115>An administrative region (markuz) of Beheira Governorate.</obo:IAO_0000115>
        <oboInOwl:hasOBONamespace>GAZ</oboInOwl:hasOBONamespace>
        <oboInOwl:id>GAZ:00066475</oboInOwl:id>
        <rdfs:label>Almahmodya Region</rdfs:label>
    </owl:NamedIndividual>
    


    <!-- http://purl.obolibrary.org/obo/GAZ_00066476 -->

    <owl:NamedIndividual rdf:about="http://purl.obolibrary.org/obo/GAZ_00066476">
        <obo:RO_0001025 rdf:resource="http://purl.obolibrary.org/obo/GAZ_00000655"/>
        <obo:IAO_0000115>An administrative region (markuz) of Beheira Governorate.</obo:IAO_0000115>
        <oboInOwl:hasOBONamespace>GAZ</oboInOwl:hasOBONamespace>
        <oboInOwl:id>GAZ:00066476</oboInOwl:id>
        <rdfs:label>Etay Elbarood Region</rdfs:label>
    </owl:NamedIndividual>
    


    <!-- http://purl.obolibrary.org/obo/GAZ_00066477 -->

    <owl:NamedIndividual rdf:about="http://purl.obolibrary.org/obo/GAZ_00066477">
        <obo:RO_0001025 rdf:resource="http://purl.obolibrary.org/obo/GAZ_00000655"/>
        <obo:IAO_0000115>An administrative region (markuz) of Beheira Governorate.</obo:IAO_0000115>
        <oboInOwl:hasOBONamespace>GAZ</oboInOwl:hasOBONamespace>
        <oboInOwl:id>GAZ:00066477</oboInOwl:id>
        <rdfs:label>Edko Region</rdfs:label>
    </owl:NamedIndividual>
    


    <!-- http://purl.obolibrary.org/obo/GAZ_00066478 -->

    <owl:NamedIndividual rdf:about="http://purl.obolibrary.org/obo/GAZ_00066478">
        <obo:RO_0001025 rdf:resource="http://purl.obolibrary.org/obo/GAZ_00000655"/>
        <obo:IAO_0000115>An administrative region (markuz) of Beheira Governorate.</obo:IAO_0000115>
        <oboInOwl:hasOBONamespace>GAZ</oboInOwl:hasOBONamespace>
        <oboInOwl:id>GAZ:00066478</oboInOwl:id>
        <rdfs:label>Alrahmanya Region</rdfs:label>
    </owl:NamedIndividual>
    


    <!-- http://purl.obolibrary.org/obo/GAZ_00066479 -->

    <owl:NamedIndividual rdf:about="http://purl.obolibrary.org/obo/GAZ_00066479">
        <obo:RO_0001025 rdf:resource="http://purl.obolibrary.org/obo/GAZ_00000655"/>
        <oboInOwl:hasOBONamespace>GAZ</oboInOwl:hasOBONamespace>
        <oboInOwl:id>GAZ:00066479</oboInOwl:id>
        <rdfs:label>Altahreer Region</rdfs:label>
    </owl:NamedIndividual>
    


    <!-- http://purl.obolibrary.org/obo/GAZ_00066480 -->

    <owl:NamedIndividual rdf:about="http://purl.obolibrary.org/obo/GAZ_00066480">
        <obo:RO_0001025 rdf:resource="http://purl.obolibrary.org/obo/GAZ_00000655"/>
        <obo:IAO_0000115>An administrative region (markuz) of Beheira Governorate.</obo:IAO_0000115>
        <oboInOwl:hasOBONamespace>GAZ</oboInOwl:hasOBONamespace>
        <oboInOwl:id>GAZ:00066480</oboInOwl:id>
        <rdfs:label>Hosheisa Region</rdfs:label>
    </owl:NamedIndividual>
    


    <!-- http://purl.obolibrary.org/obo/GAZ_00066481 -->

    <owl:NamedIndividual rdf:about="http://purl.obolibrary.org/obo/GAZ_00066481">
        <obo:RO_0001025 rdf:resource="http://purl.obolibrary.org/obo/GAZ_00000655"/>
        <obo:IAO_0000115>An administrative region (markuz) of Beheira Governorate.</obo:IAO_0000115>
        <oboInOwl:hasOBONamespace>GAZ</oboInOwl:hasOBONamespace>
        <oboInOwl:id>GAZ:00066481</oboInOwl:id>
        <rdfs:label>Kom Hamada Region</rdfs:label>
    </owl:NamedIndividual>
    


    <!-- http://purl.obolibrary.org/obo/GAZ_00066482 -->

    <owl:NamedIndividual rdf:about="http://purl.obolibrary.org/obo/GAZ_00066482">
        <obo:RO_0001025 rdf:resource="http://purl.obolibrary.org/obo/GAZ_00000655"/>
        <obo:IAO_0000115>An administrative region (markuz) of Beheira Governorate.</obo:IAO_0000115>
        <oboInOwl:hasOBONamespace>GAZ</oboInOwl:hasOBONamespace>
        <oboInOwl:id>GAZ:00066482</oboInOwl:id>
        <rdfs:label>Shobrakheet Region</rdfs:label>
    </owl:NamedIndividual>
    


    <!-- http://purl.obolibrary.org/obo/GAZ_00066483 -->

    <owl:NamedIndividual rdf:about="http://purl.obolibrary.org/obo/GAZ_00066483">
        <obo:RO_0001025 rdf:resource="http://purl.obolibrary.org/obo/GAZ_00000655"/>
        <obo:IAO_0000115>An administrative region (markuz) of Beheira Governorate.</obo:IAO_0000115>
        <oboInOwl:hasOBONamespace>GAZ</oboInOwl:hasOBONamespace>
        <oboInOwl:id>GAZ:00066483</oboInOwl:id>
        <rdfs:label>Kafr Eldawar Region</rdfs:label>
    </owl:NamedIndividual>
    


    <!-- http://purl.obolibrary.org/obo/GAZ_00066485 -->

    <owl:NamedIndividual rdf:about="http://purl.obolibrary.org/obo/GAZ_00066485">
        <obo:RO_0001025 rdf:resource="http://purl.obolibrary.org/obo/GAZ_00005648"/>
        <obo:IAO_0000115>An administrative region (kism) of Cairo Governorate.</obo:IAO_0000115>
        <oboInOwl:hasOBONamespace>GAZ</oboInOwl:hasOBONamespace>
        <oboInOwl:id>GAZ:00066485</oboInOwl:id>
        <rdfs:label>Kism Hdaak El Koba</rdfs:label>
    </owl:NamedIndividual>
    


    <!-- http://purl.obolibrary.org/obo/GAZ_00066488 -->

    <owl:NamedIndividual rdf:about="http://purl.obolibrary.org/obo/GAZ_00066488">
        <obo:RO_0001025 rdf:resource="http://purl.obolibrary.org/obo/GAZ_00005648"/>
        <obo:IAO_0000115>An administrative region (kism) of Cairo Governorate.</obo:IAO_0000115>
        <oboInOwl:hasOBONamespace>GAZ</oboInOwl:hasOBONamespace>
        <oboInOwl:id>GAZ:00066488</oboInOwl:id>
        <rdfs:label>Kism Shubra</rdfs:label>
    </owl:NamedIndividual>
    


    <!-- http://purl.obolibrary.org/obo/GAZ_00066491 -->

    <owl:NamedIndividual rdf:about="http://purl.obolibrary.org/obo/GAZ_00066491">
        <obo:RO_0001025 rdf:resource="http://purl.obolibrary.org/obo/GAZ_00005648"/>
        <obo:IAO_0000115>An administrative region (kism) of Cairo Governorate.</obo:IAO_0000115>
        <oboInOwl:hasOBONamespace>GAZ</oboInOwl:hasOBONamespace>
        <oboInOwl:id>GAZ:00066491</oboInOwl:id>
        <rdfs:label>Kism Monshat Nasr</rdfs:label>
    </owl:NamedIndividual>
    


    <!-- http://purl.obolibrary.org/obo/GAZ_00066492 -->

    <owl:NamedIndividual rdf:about="http://purl.obolibrary.org/obo/GAZ_00066492">
        <obo:RO_0001025 rdf:resource="http://purl.obolibrary.org/obo/GAZ_00005648"/>
        <obo:IAO_0000115>An administrative region (kism) of Cairo Governorate.</obo:IAO_0000115>
        <oboInOwl:hasOBONamespace>GAZ</oboInOwl:hasOBONamespace>
        <oboInOwl:id>GAZ:00066492</oboInOwl:id>
        <rdfs:label>Kism Bab El Sharia</rdfs:label>
    </owl:NamedIndividual>
    


    <!-- http://purl.obolibrary.org/obo/GAZ_00066494 -->

    <owl:NamedIndividual rdf:about="http://purl.obolibrary.org/obo/GAZ_00066494">
        <obo:RO_0001025 rdf:resource="http://purl.obolibrary.org/obo/GAZ_00005648"/>
        <obo:IAO_0000115>An administrative region (kism) of Cairo Governorate.</obo:IAO_0000115>
        <oboInOwl:hasOBONamespace>GAZ</oboInOwl:hasOBONamespace>
        <oboInOwl:id>GAZ:00066494</oboInOwl:id>
        <rdfs:label>Kism As Sayyidah Zaynab</rdfs:label>
    </owl:NamedIndividual>
    


    <!-- http://purl.obolibrary.org/obo/GAZ_00066495 -->

    <owl:NamedIndividual rdf:about="http://purl.obolibrary.org/obo/GAZ_00066495">
        <obo:RO_0001025 rdf:resource="http://purl.obolibrary.org/obo/GAZ_00005648"/>
        <obo:IAO_0000115>An administrative region (kism) of Cairo Governorate.</obo:IAO_0000115>
        <oboInOwl:hasOBONamespace>GAZ</oboInOwl:hasOBONamespace>
        <oboInOwl:id>GAZ:00066495</oboInOwl:id>
        <rdfs:label>Kism El Salam</rdfs:label>
    </owl:NamedIndividual>
    


    <!-- http://purl.obolibrary.org/obo/GAZ_00066496 -->

    <owl:NamedIndividual rdf:about="http://purl.obolibrary.org/obo/GAZ_00066496">
        <obo:RO_0001025 rdf:resource="http://purl.obolibrary.org/obo/GAZ_00005648"/>
        <obo:IAO_0000115>An administrative region (kism) of Cairo Governorate.</obo:IAO_0000115>
        <oboInOwl:hasOBONamespace>GAZ</oboInOwl:hasOBONamespace>
        <oboInOwl:id>GAZ:00066496</oboInOwl:id>
        <rdfs:label>Kism Rawd al Faraj</rdfs:label>
    </owl:NamedIndividual>
    


    <!-- http://purl.obolibrary.org/obo/GAZ_00066498 -->

    <owl:NamedIndividual rdf:about="http://purl.obolibrary.org/obo/GAZ_00066498">
        <obo:RO_0001025 rdf:resource="http://purl.obolibrary.org/obo/GAZ_00005648"/>
        <obo:IAO_0000115>An administrative region (kism) of Cairo Governorate.</obo:IAO_0000115>
        <oboInOwl:hasOBONamespace>GAZ</oboInOwl:hasOBONamespace>
        <oboInOwl:id>GAZ:00066498</oboInOwl:id>
        <rdfs:label>Kism Al Marj</rdfs:label>
    </owl:NamedIndividual>
    


    <!-- http://purl.obolibrary.org/obo/GAZ_00066499 -->

    <owl:NamedIndividual rdf:about="http://purl.obolibrary.org/obo/GAZ_00066499">
        <obo:RO_0001025 rdf:resource="http://purl.obolibrary.org/obo/GAZ_00230304"/>
        <obo:IAO_0000115>An administrative region (kism) of Helwan Governorate.</obo:IAO_0000115>
        <oboInOwl:hasOBONamespace>GAZ</oboInOwl:hasOBONamespace>
        <oboInOwl:id>GAZ:00066499</oboInOwl:id>
        <rdfs:label>Kism Hulwan</rdfs:label>
    </owl:NamedIndividual>
    


    <!-- http://purl.obolibrary.org/obo/GAZ_00066500 -->

    <owl:NamedIndividual rdf:about="http://purl.obolibrary.org/obo/GAZ_00066500">
        <obo:RO_0001025 rdf:resource="http://purl.obolibrary.org/obo/GAZ_00005648"/>
        <obo:IAO_0000115>An administrative region (kism) of Cairo Governorate.</obo:IAO_0000115>
        <oboInOwl:hasOBONamespace>GAZ</oboInOwl:hasOBONamespace>
        <oboInOwl:id>GAZ:00066500</oboInOwl:id>
        <rdfs:label>Kism Ein Shams</rdfs:label>
    </owl:NamedIndividual>
    


    <!-- http://purl.obolibrary.org/obo/GAZ_00066501 -->

    <owl:NamedIndividual rdf:about="http://purl.obolibrary.org/obo/GAZ_00066501">
        <obo:RO_0001025 rdf:resource="http://purl.obolibrary.org/obo/GAZ_00005648"/>
        <obo:IAO_0000115>An administrative region (kism) of Cairo Governorate.</obo:IAO_0000115>
        <oboInOwl:hasOBONamespace>GAZ</oboInOwl:hasOBONamespace>
        <oboInOwl:id>GAZ:00066501</oboInOwl:id>
        <rdfs:label>Kism El Waily</rdfs:label>
    </owl:NamedIndividual>
    


    <!-- http://purl.obolibrary.org/obo/GAZ_00066502 -->

    <owl:NamedIndividual rdf:about="http://purl.obolibrary.org/obo/GAZ_00066502">
        <obo:RO_0001025 rdf:resource="http://purl.obolibrary.org/obo/GAZ_00005648"/>
        <obo:IAO_0000115>An administrative region (kism) of Cairo Governorate.</obo:IAO_0000115>
        <oboInOwl:hasOBONamespace>GAZ</oboInOwl:hasOBONamespace>
        <oboInOwl:id>GAZ:00066502</oboInOwl:id>
        <rdfs:label>Kism El Sahel</rdfs:label>
    </owl:NamedIndividual>
    


    <!-- http://purl.obolibrary.org/obo/GAZ_00066503 -->

    <owl:NamedIndividual rdf:about="http://purl.obolibrary.org/obo/GAZ_00066503">
        <obo:RO_0001025 rdf:resource="http://purl.obolibrary.org/obo/GAZ_00005648"/>
        <obo:IAO_0000115>An administrative region (kism) of Cairo Governorate.</obo:IAO_0000115>
        <oboInOwl:hasOBONamespace>GAZ</oboInOwl:hasOBONamespace>
        <oboInOwl:id>GAZ:00066503</oboInOwl:id>
        <rdfs:label>Kism El Zayton</rdfs:label>
    </owl:NamedIndividual>
    


    <!-- http://purl.obolibrary.org/obo/GAZ_00066504 -->

    <owl:NamedIndividual rdf:about="http://purl.obolibrary.org/obo/GAZ_00066504">
        <obo:RO_0001025 rdf:resource="http://purl.obolibrary.org/obo/GAZ_00005648"/>
        <obo:IAO_0000115>An administrative region (kism) of Cairo Governorate.</obo:IAO_0000115>
        <oboInOwl:hasOBONamespace>GAZ</oboInOwl:hasOBONamespace>
        <oboInOwl:id>GAZ:00066504</oboInOwl:id>
        <rdfs:label>Kism Elsharabia</rdfs:label>
    </owl:NamedIndividual>
    


    <!-- http://purl.obolibrary.org/obo/GAZ_00066506 -->

    <owl:NamedIndividual rdf:about="http://purl.obolibrary.org/obo/GAZ_00066506">
        <obo:RO_0001025 rdf:resource="http://purl.obolibrary.org/obo/GAZ_00005648"/>
        <obo:IAO_0000115>An administrative region (kism) of Cairo Governorate.</obo:IAO_0000115>
        <oboInOwl:hasOBONamespace>GAZ</oboInOwl:hasOBONamespace>
        <oboInOwl:id>GAZ:00066506</oboInOwl:id>
        <rdfs:label>Kism Al Matariyah</rdfs:label>
    </owl:NamedIndividual>
    


    <!-- http://purl.obolibrary.org/obo/GAZ_00066507 -->

    <owl:NamedIndividual rdf:about="http://purl.obolibrary.org/obo/GAZ_00066507">
        <obo:RO_0001025 rdf:resource="http://purl.obolibrary.org/obo/GAZ_00005648"/>
        <obo:IAO_0000115>An administrative region (kism) of Cairo Governorate.</obo:IAO_0000115>
        <oboInOwl:hasOBONamespace>GAZ</oboInOwl:hasOBONamespace>
        <oboInOwl:id>GAZ:00066507</oboInOwl:id>
        <rdfs:label>Kism Abdin</rdfs:label>
    </owl:NamedIndividual>
    


    <!-- http://purl.obolibrary.org/obo/GAZ_00076360 -->

    <owl:NamedIndividual rdf:about="http://purl.obolibrary.org/obo/GAZ_00076360">
        <obo:RO_0001025 rdf:resource="http://purl.obolibrary.org/obo/GAZ_00000670"/>
        <obo:IAO_0000115>A national park. Established 1988.</obo:IAO_0000115>
        <oboInOwl:hasOBONamespace>GAZ</oboInOwl:hasOBONamespace>
        <oboInOwl:id>GAZ:00076360</oboInOwl:id>
        <rdfs:label>Saint Catherine National Park</rdfs:label>
    </owl:NamedIndividual>
    


    <!-- http://purl.obolibrary.org/obo/GAZ_00076361 -->

    <owl:NamedIndividual rdf:about="http://purl.obolibrary.org/obo/GAZ_00076361">
        <obo:RO_0001025 rdf:resource="http://purl.obolibrary.org/obo/GAZ_00000668"/>
        <obo:IAO_0000115>A national park.</obo:IAO_0000115>
        <oboInOwl:hasOBONamespace>GAZ</oboInOwl:hasOBONamespace>
        <oboInOwl:id>GAZ:00076361</oboInOwl:id>
        <rdfs:label>Wadi el Gamal National Park</rdfs:label>
    </owl:NamedIndividual>
    


    <!-- http://purl.obolibrary.org/obo/GAZ_00089761 -->

    <owl:NamedIndividual rdf:about="http://purl.obolibrary.org/obo/GAZ_00089761">
        <obo:RO_0001025 rdf:resource="http://purl.obolibrary.org/obo/GAZ_00000669"/>
        <obo:IAO_0000115>A wetland protected area. Established 1985.</obo:IAO_0000115>
        <oboInOwl:hasOBONamespace>GAZ</oboInOwl:hasOBONamespace>
        <oboInOwl:id>GAZ:00089761</oboInOwl:id>
        <rdfs:label>Zaranik Protected Area</rdfs:label>
    </owl:NamedIndividual>
    


    <!-- http://purl.obolibrary.org/obo/GAZ_00089762 -->

    <owl:NamedIndividual rdf:about="http://purl.obolibrary.org/obo/GAZ_00089762">
        <obo:RO_0001025 rdf:resource="http://purl.obolibrary.org/obo/GAZ_00000670"/>
        <obo:IAO_0000115>A protected area located at the meeting point of the Gulf of Suez and Aqaba Gulf. The Eastern border of Ras Mohamed Protected Area is a rocky wall with the gulf water where there are coral reefs. There is also the Mangrove channel which separates Ras Mohamed Peninsula from Elbayra Island at a length of approximately 250 m. Establishd 1983.</obo:IAO_0000115>
        <oboInOwl:hasOBONamespace>GAZ</oboInOwl:hasOBONamespace>
        <oboInOwl:id>GAZ:00089762</oboInOwl:id>
        <rdfs:label>Ras Mohamed Protected Area</rdfs:label>
    </owl:NamedIndividual>
    


    <!-- http://purl.obolibrary.org/obo/GAZ_00089763 -->

    <owl:NamedIndividual rdf:about="http://purl.obolibrary.org/obo/GAZ_00089763">
        <obo:RO_0001025 rdf:resource="http://purl.obolibrary.org/obo/GAZ_00000669"/>
        <obo:IAO_0000115>A protected area of coastal marshes. Established in 1985.</obo:IAO_0000115>
        <oboInOwl:hasOBONamespace>GAZ</oboInOwl:hasOBONamespace>
        <oboInOwl:id>GAZ:00089763</oboInOwl:id>
        <rdfs:label>Ahrash Protectorate</rdfs:label>
    </owl:NamedIndividual>
    


    <!-- http://purl.obolibrary.org/obo/GAZ_00089764 -->

    <owl:NamedIndividual rdf:about="http://purl.obolibrary.org/obo/GAZ_00089764">
        <obo:RO_0001025 rdf:resource="http://purl.obolibrary.org/obo/GAZ_00000654"/>
        <obo:IAO_0000115>A protected area located in the southern eastern part of the eastern desert. Its mountains are located on the joint borders of Egypt and the Sudan on the Red Sea. Established 1986.</obo:IAO_0000115>
        <oboInOwl:hasOBONamespace>GAZ</oboInOwl:hasOBONamespace>
        <oboInOwl:id>GAZ:00089764</oboInOwl:id>
        <rdfs:label>Elba Natural Protected Area</rdfs:label>
    </owl:NamedIndividual>
    


    <!-- http://purl.obolibrary.org/obo/GAZ_00089765 -->

    <owl:NamedIndividual rdf:about="http://purl.obolibrary.org/obo/GAZ_00089765">
        <obo:RO_0001025 rdf:resource="http://purl.obolibrary.org/obo/GAZ_00000667"/>
        <obo:IAO_0000115>A protected area established in 1986.</obo:IAO_0000115>
        <oboInOwl:hasOBONamespace>GAZ</oboInOwl:hasOBONamespace>
        <oboInOwl:id>GAZ:00089765</oboInOwl:id>
        <rdfs:label>Elomayed Natural Protected Area</rdfs:label>
    </owl:NamedIndividual>
    


    <!-- http://purl.obolibrary.org/obo/GAZ_00089766 -->

    <owl:NamedIndividual rdf:about="http://purl.obolibrary.org/obo/GAZ_00089766">
        <obo:RO_0001025 rdf:resource="http://purl.obolibrary.org/obo/GAZ_00000645"/>
        <obo:IAO_0000115>A protected area including Saloga, Ghazal and the small Islands in between (First Cataract). Established in 1986.</obo:IAO_0000115>
        <oboInOwl:hasOBONamespace>GAZ</oboInOwl:hasOBONamespace>
        <oboInOwl:id>GAZ:00089766</oboInOwl:id>
        <rdfs:label>Saluga and Ghazal Protectorate</rdfs:label>
    </owl:NamedIndividual>
    


    <!-- http://purl.obolibrary.org/obo/GAZ_00089767 -->

    <owl:NamedIndividual rdf:about="http://purl.obolibrary.org/obo/GAZ_00089767">
        <obo:RO_0001025 rdf:resource="http://purl.obolibrary.org/obo/GAZ_00000665"/>
        <obo:IAO_0000115>A protected area that includes the bays of El Gamil and Ashtoon El Gamil and Al Manzala lagoon. Tenis island is located in El Manzala lagoon. Established in 1988.</obo:IAO_0000115>
        <oboInOwl:hasOBONamespace>GAZ</oboInOwl:hasOBONamespace>
        <oboInOwl:id>GAZ:00089767</oboInOwl:id>
        <rdfs:label>Ashtum El Gamil Protectorate</rdfs:label>
    </owl:NamedIndividual>
    


    <!-- http://purl.obolibrary.org/obo/GAZ_00089768 -->

    <owl:NamedIndividual rdf:about="http://purl.obolibrary.org/obo/GAZ_00089768">
        <obo:RO_0001025 rdf:resource="http://purl.obolibrary.org/obo/GAZ_00058845"/>
        <obo:IAO_0000115>An island in Lake Manzala.</obo:IAO_0000115>
        <oboInOwl:hasOBONamespace>GAZ</oboInOwl:hasOBONamespace>
        <oboInOwl:id>GAZ:00089768</oboInOwl:id>
        <rdfs:label>Tenis Island</rdfs:label>
    </owl:NamedIndividual>
    


    <!-- http://purl.obolibrary.org/obo/GAZ_00089769 -->

    <owl:NamedIndividual rdf:about="http://purl.obolibrary.org/obo/GAZ_00089769">
        <obo:RO_0001025 rdf:resource="http://purl.obolibrary.org/obo/GAZ_00230318"/>
        <obo:IAO_0000115>A protected area that includes a large dry river that used to rise from the Red Sea hills especially Elba mountain. After the construction of the High Dam and filling lake Naser with water, the water flowed into Wadi Al -Alaqi and it became part of the Lake. Established 1989.</obo:IAO_0000115>
        <oboInOwl:hasOBONamespace>GAZ</oboInOwl:hasOBONamespace>
        <oboInOwl:id>GAZ:00089769</oboInOwl:id>
        <rdfs:label>Wadi Alaqi Protectorate</rdfs:label>
    </owl:NamedIndividual>
    


    <!-- http://purl.obolibrary.org/obo/GAZ_00089770 -->

    <owl:NamedIndividual rdf:about="http://purl.obolibrary.org/obo/GAZ_00089770">
        <obo:RO_0001025 rdf:resource="http://purl.obolibrary.org/obo/GAZ_00089771"/>
        <obo:IAO_0000115>A protected area. Established in 1989.</obo:IAO_0000115>
        <oboInOwl:hasOBONamespace>GAZ</oboInOwl:hasOBONamespace>
        <oboInOwl:id>GAZ:00089770</oboInOwl:id>
        <rdfs:label>Petrified Forest Protectorate</rdfs:label>
    </owl:NamedIndividual>
    


    <!-- http://purl.obolibrary.org/obo/GAZ_00089771 -->

    <owl:NamedIndividual rdf:about="http://purl.obolibrary.org/obo/GAZ_00089771">
        <obo:RO_0001025 rdf:resource="http://purl.obolibrary.org/obo/GAZ_00242103"/>
    </owl:NamedIndividual>
    


    <!-- http://purl.obolibrary.org/obo/GAZ_00089772 -->

    <owl:NamedIndividual rdf:about="http://purl.obolibrary.org/obo/GAZ_00089772">
        <obo:RO_0001025 rdf:resource="http://purl.obolibrary.org/obo/GAZ_00000646"/>
        <obo:IAO_0000115>A protected area established in 1989.</obo:IAO_0000115>
        <oboInOwl:hasOBONamespace>GAZ</oboInOwl:hasOBONamespace>
        <oboInOwl:id>GAZ:00089772</oboInOwl:id>
        <rdfs:label>Wadi El Assuti Protectorate</rdfs:label>
    </owl:NamedIndividual>
    


    <!-- http://purl.obolibrary.org/obo/GAZ_00089773 -->

    <owl:NamedIndividual rdf:about="http://purl.obolibrary.org/obo/GAZ_00089773">
        <obo:RO_0001025 rdf:resource="http://purl.obolibrary.org/obo/GAZ_00000648"/>
        <obo:IAO_0000115>A protected area. Established 1989.</obo:IAO_0000115>
        <oboInOwl:hasOBONamespace>GAZ</oboInOwl:hasOBONamespace>
        <oboInOwl:id>GAZ:00089773</oboInOwl:id>
        <rdfs:label>Wadi El Rayan Protectorate</rdfs:label>
    </owl:NamedIndividual>
    


    <!-- http://purl.obolibrary.org/obo/GAZ_00089774 -->

    <owl:NamedIndividual rdf:about="http://purl.obolibrary.org/obo/GAZ_00089774">
        <obo:RO_0001025 rdf:resource="http://purl.obolibrary.org/obo/GAZ_00066385"/>
        <obo:IAO_0000115>A protected area. Established 1989.</obo:IAO_0000115>
        <oboInOwl:hasOBONamespace>GAZ</oboInOwl:hasOBONamespace>
        <oboInOwl:id>GAZ:00089774</oboInOwl:id>
        <rdfs:label>Lake Qarun Protectorate</rdfs:label>
    </owl:NamedIndividual>
    


    <!-- http://purl.obolibrary.org/obo/GAZ_00089775 -->

    <owl:NamedIndividual rdf:about="http://purl.obolibrary.org/obo/GAZ_00089775">
        <obo:RO_0001025 rdf:resource="http://purl.obolibrary.org/obo/GAZ_00000649"/>
        <obo:IAO_0000115>A protected area. Established in 1989.</obo:IAO_0000115>
        <oboInOwl:hasOBONamespace>GAZ</oboInOwl:hasOBONamespace>
        <oboInOwl:id>GAZ:00089775</oboInOwl:id>
        <rdfs:label>El Hassana Dome Protectorate</rdfs:label>
    </owl:NamedIndividual>
    


    <!-- http://purl.obolibrary.org/obo/GAZ_00089776 -->

    <owl:NamedIndividual rdf:about="http://purl.obolibrary.org/obo/GAZ_00089776">
        <obo:RO_0001025 rdf:resource="http://purl.obolibrary.org/obo/GAZ_00000647"/>
        <obo:IAO_0000115>A protected area established in 1992.</obo:IAO_0000115>
        <oboInOwl:hasOBONamespace>GAZ</oboInOwl:hasOBONamespace>
        <oboInOwl:id>GAZ:00089776</oboInOwl:id>
        <rdfs:label>Sannur Cave Protectorate</rdfs:label>
    </owl:NamedIndividual>
    


    <!-- http://purl.obolibrary.org/obo/GAZ_00089777 -->

    <owl:NamedIndividual rdf:about="http://purl.obolibrary.org/obo/GAZ_00089777">
        <obo:RO_0001025 rdf:resource="http://purl.obolibrary.org/obo/GAZ_00089776"/>
        <oboInOwl:hasOBONamespace>GAZ</oboInOwl:hasOBONamespace>
        <oboInOwl:id>GAZ:00089777</oboInOwl:id>
        <rdfs:label>Wadi Sanor Cave</rdfs:label>
    </owl:NamedIndividual>
    


    <!-- http://purl.obolibrary.org/obo/GAZ_00089778 -->

    <owl:NamedIndividual rdf:about="http://purl.obolibrary.org/obo/GAZ_00089778">
        <obo:RO_0001025 rdf:resource="http://purl.obolibrary.org/obo/GAZ_00000670"/>
        <obo:IAO_0000115>A protected area established in 1992.</obo:IAO_0000115>
        <oboInOwl:hasOBONamespace>GAZ</oboInOwl:hasOBONamespace>
        <oboInOwl:id>GAZ:00089778</oboInOwl:id>
        <rdfs:label>Nabaq Protectorate</rdfs:label>
    </owl:NamedIndividual>
    


    <!-- http://purl.obolibrary.org/obo/GAZ_00089779 -->

    <owl:NamedIndividual rdf:about="http://purl.obolibrary.org/obo/GAZ_00089779">
        <obo:RO_0001025 rdf:resource="http://purl.obolibrary.org/obo/GAZ_00000670"/>
        <obo:IAO_0000115>A protected area established in 1992.</obo:IAO_0000115>
        <oboInOwl:hasOBONamespace>GAZ</oboInOwl:hasOBONamespace>
        <oboInOwl:id>GAZ:00089779</oboInOwl:id>
        <rdfs:label>Abu Galum Protectorate</rdfs:label>
    </owl:NamedIndividual>
    


    <!-- http://purl.obolibrary.org/obo/GAZ_00089780 -->

    <owl:NamedIndividual rdf:about="http://purl.obolibrary.org/obo/GAZ_00089780">
        <obo:RO_0001025 rdf:resource="http://purl.obolibrary.org/obo/GAZ_00000670"/>
        <obo:IAO_0000115>A protected area established in 1998.</obo:IAO_0000115>
        <oboInOwl:hasOBONamespace>GAZ</oboInOwl:hasOBONamespace>
        <oboInOwl:id>GAZ:00089780</oboInOwl:id>
        <rdfs:label>Taba Protectorate</rdfs:label>
    </owl:NamedIndividual>
    


    <!-- http://purl.obolibrary.org/obo/GAZ_00089781 -->

    <owl:NamedIndividual rdf:about="http://purl.obolibrary.org/obo/GAZ_00089781">
        <obo:RO_0001025 rdf:resource="http://purl.obolibrary.org/obo/GAZ_00000659"/>
        <obo:IAO_0000115>A protected area established in 1998.</obo:IAO_0000115>
        <oboInOwl:hasOBONamespace>GAZ</oboInOwl:hasOBONamespace>
        <oboInOwl:id>GAZ:00089781</oboInOwl:id>
        <rdfs:label>Lake Burullus Protectorate</rdfs:label>
    </owl:NamedIndividual>
    


    <!-- http://purl.obolibrary.org/obo/GAZ_00089782 -->

    <owl:NamedIndividual rdf:about="http://purl.obolibrary.org/obo/GAZ_00089782">
        <obo:IAO_0000115>Protected areas amounting to 144 islands in different Governorates in Egypt. Alongside the main stream from Aswan until the Barrages, there are 95 Islands within an area of 32500 Feddans. In Rasheed branch there are 30 islands within an area of 3400 Feddans, in Damietta Branch there are 19 islands within and area of 1250 Feddans. The total area of all the Nile River islands in 37150 Feddans.</obo:IAO_0000115>
        <oboInOwl:hasOBONamespace>GAZ</oboInOwl:hasOBONamespace>
        <oboInOwl:id>GAZ:00089782</oboInOwl:id>
        <rdfs:label>Nile river Islands Protected Area</rdfs:label>
    </owl:NamedIndividual>
    


    <!-- http://purl.obolibrary.org/obo/GAZ_00089783 -->

    <owl:NamedIndividual rdf:about="http://purl.obolibrary.org/obo/GAZ_00089783">
        <obo:RO_0001025 rdf:resource="http://purl.obolibrary.org/obo/GAZ_00000663"/>
        <obo:IAO_0000115>A protected area for the Wadi Digla, one of the important valleys which extend from east to west with a length of 30 km.</obo:IAO_0000115>
        <oboInOwl:hasOBONamespace>GAZ</oboInOwl:hasOBONamespace>
        <oboInOwl:id>GAZ:00089783</oboInOwl:id>
        <rdfs:label>Wadi Digla Protectorate</rdfs:label>
    </owl:NamedIndividual>
    


    <!-- http://purl.obolibrary.org/obo/GAZ_00089784 -->

    <owl:NamedIndividual rdf:about="http://purl.obolibrary.org/obo/GAZ_00089784">
        <obo:RO_0001025 rdf:resource="http://purl.obolibrary.org/obo/GAZ_00000667"/>
        <obo:IAO_0000115>A protected area established in 2002.</obo:IAO_0000115>
        <oboInOwl:hasOBONamespace>GAZ</oboInOwl:hasOBONamespace>
        <oboInOwl:id>GAZ:00089784</oboInOwl:id>
        <rdfs:label>Natural Siwa Protected Area</rdfs:label>
    </owl:NamedIndividual>
    


    <!-- http://purl.obolibrary.org/obo/GAZ_00089785 -->

    <owl:NamedIndividual rdf:about="http://purl.obolibrary.org/obo/GAZ_00089785">
        <obo:RO_0001025 rdf:resource="http://purl.obolibrary.org/obo/GAZ_00000654"/>
        <obo:IAO_0000115>A protected area established in 2003. It includes the segment of the Red Sea coastal plain and mountains extending roughly between 24deg51minN in the north and 24deg06minN in the south; and between the Red Sea shoreline in the east to about 34deg28minE in the west (the Sheikh Shazli road). The protected area also encompasses a section of the marine environment including the islands of Hamata and Wadi El Gemal Island.</obo:IAO_0000115>
        <oboInOwl:hasOBONamespace>GAZ</oboInOwl:hasOBONamespace>
        <oboInOwl:id>GAZ:00089785</oboInOwl:id>
        <rdfs:label>Wadi El Gemal - Hamata Protected Area</rdfs:label>
    </owl:NamedIndividual>
    


    <!-- http://purl.obolibrary.org/obo/GAZ_00089786 -->

    <owl:NamedIndividual rdf:about="http://purl.obolibrary.org/obo/GAZ_00089786">
        <obo:RO_0001025 rdf:resource="http://purl.obolibrary.org/obo/GAZ_00000668"/>
        <obo:IAO_0000115>A protected area in El Wady EL Gedid.</obo:IAO_0000115>
        <oboInOwl:hasOBONamespace>GAZ</oboInOwl:hasOBONamespace>
        <oboInOwl:id>GAZ:00089786</oboInOwl:id>
        <rdfs:label>Natural White Desert Protected Area</rdfs:label>
    </owl:NamedIndividual>
    


    <!-- http://purl.obolibrary.org/obo/GAZ_00102117 -->

    <owl:NamedIndividual rdf:about="http://purl.obolibrary.org/obo/GAZ_00102117">
        <obo:RO_0001025 rdf:resource="http://purl.obolibrary.org/obo/GAZ_00051269"/>
        <obo:IAO_0000115>The eastern side (3 km wide and 30 m deep) of the Bab-el-Mandeb straits separating Ras Menheli, Yemen, on the Arabian Peninsula and Ras Siyan, Djibouti, on the Horn of Africa. The Yemeni island of Perim divides the strait into two channels.</obo:IAO_0000115>
        <oboInOwl:hasOBONamespace>GAZ</oboInOwl:hasOBONamespace>
        <oboInOwl:id>GAZ:00102117</oboInOwl:id>
        <rdfs:label>Bab Iskender</rdfs:label>
    </owl:NamedIndividual>
    


    <!-- http://purl.obolibrary.org/obo/GAZ_00102118 -->

    <owl:NamedIndividual rdf:about="http://purl.obolibrary.org/obo/GAZ_00102118">
        <obo:RO_0001025 rdf:resource="http://purl.obolibrary.org/obo/GAZ_00051269"/>
        <obo:IAO_0000115>The western side of the Bab-el-Mandeb strait.</obo:IAO_0000115>
        <oboInOwl:hasOBONamespace>GAZ</oboInOwl:hasOBONamespace>
        <oboInOwl:id>GAZ:00102118</oboInOwl:id>
        <rdfs:label>Dact-el-Mayun</rdfs:label>
    </owl:NamedIndividual>
    


    <!-- http://purl.obolibrary.org/obo/GAZ_00103898 -->

    <owl:NamedIndividual rdf:about="http://purl.obolibrary.org/obo/GAZ_00103898">
        <obo:IAO_0000115>A triangular massif, located in northern Niger, within the Sahara desert. Part of the West Saharan montane xeric woodlands ecoregion, they rise to more than 1,830 m and extend over 84000 km2. Lying in the midst of desert north of the 17th parallel, the Air plateau with an average altitude between 500 and 900 m, forms an island of Sahel climate.</obo:IAO_0000115>
        <oboInOwl:hasOBONamespace>GAZ</oboInOwl:hasOBONamespace>
        <oboInOwl:id>GAZ:00103898</oboInOwl:id>
        <rdfs:label>Air Mountains</rdfs:label>
    </owl:NamedIndividual>
    


    <!-- http://purl.obolibrary.org/obo/GAZ_00122801 -->

    <owl:NamedIndividual rdf:about="http://purl.obolibrary.org/obo/GAZ_00122801">
        <obo:IAO_0000115>A depression located at the southern edge of the Sahara Desert in north central Africa, is the lowest point in Chad, and one of the largest sources of airborne dust in the world. Once serving as part of the floor of a much larger Lake Chad.</obo:IAO_0000115>
        <oboInOwl:hasOBONamespace>GAZ</oboInOwl:hasOBONamespace>
        <oboInOwl:id>GAZ:00122801</oboInOwl:id>
        <rdfs:label>Bodele Depression</rdfs:label>
    </owl:NamedIndividual>
    


    <!-- http://purl.obolibrary.org/obo/GAZ_00144637 -->

    <owl:NamedIndividual rdf:about="http://purl.obolibrary.org/obo/GAZ_00144637">
        <obo:RO_0001025 rdf:resource="http://purl.obolibrary.org/obo/GAZ_00000654"/>
        <obo:RO_0001025 rdf:resource="http://purl.obolibrary.org/obo/GAZ_00002456"/>
        <obo:IAO_0000115>An inlet of water on the Egyptian side of the Red Sea. It is located slightly north of the Tropic of Cancer. The northern part of Foul Bay is the Ras Banas peninsula.</obo:IAO_0000115>
        <oboInOwl:hasOBONamespace>GAZ</oboInOwl:hasOBONamespace>
        <oboInOwl:id>GAZ:00144637</oboInOwl:id>
        <rdfs:label>Foul Bay</rdfs:label>
    </owl:NamedIndividual>
    


    <!-- http://purl.obolibrary.org/obo/GAZ_00144638 -->

    <owl:NamedIndividual rdf:about="http://purl.obolibrary.org/obo/GAZ_00144638">
        <obo:RO_0001025 rdf:resource="http://purl.obolibrary.org/obo/GAZ_00144637"/>
        <obo:IAO_0000115>An island in Foul Bay.</obo:IAO_0000115>
        <oboInOwl:hasOBONamespace>GAZ</oboInOwl:hasOBONamespace>
        <oboInOwl:id>GAZ:00144638</oboInOwl:id>
        <rdfs:label>Rocky Island</rdfs:label>
    </owl:NamedIndividual>
    


    <!-- http://purl.obolibrary.org/obo/GAZ_00144639 -->

    <owl:NamedIndividual rdf:about="http://purl.obolibrary.org/obo/GAZ_00144639">
        <obo:RO_0001025 rdf:resource="http://purl.obolibrary.org/obo/GAZ_00144637"/>
        <obo:IAO_0000115>The largest of a group of islands in Foul Bay, Red Sea in Southern Egypt.</obo:IAO_0000115>
        <oboInOwl:hasOBONamespace>GAZ</oboInOwl:hasOBONamespace>
        <oboInOwl:id>GAZ:00144639</oboInOwl:id>
        <rdfs:label>Saint John&apos;s Island</rdfs:label>
    </owl:NamedIndividual>
    


    <!-- http://purl.obolibrary.org/obo/GAZ_00145311 -->

    <owl:NamedIndividual rdf:about="http://purl.obolibrary.org/obo/GAZ_00145311">
        <obo:RO_0001025 rdf:resource="http://purl.obolibrary.org/obo/GAZ_00002456"/>
        <obo:IAO_0000115>A body of water on the Eritrean coastline on the Red Sea. The Gulf lies near the midpoint of the Eritrean coast, between the Foro province and the Buri Peninsula of the Ghelae&apos;lo province, both in the country&apos;s Northern Red Sea region.</obo:IAO_0000115>
        <oboInOwl:hasOBONamespace>GAZ</oboInOwl:hasOBONamespace>
        <oboInOwl:id>GAZ:00145311</oboInOwl:id>
        <rdfs:label>Gulf of Zula</rdfs:label>
    </owl:NamedIndividual>
    


    <!-- http://purl.obolibrary.org/obo/GAZ_00146201 -->

    <owl:NamedIndividual rdf:about="http://purl.obolibrary.org/obo/GAZ_00146201">
        <obo:RO_0001025 rdf:resource="http://purl.obolibrary.org/obo/GAZ_00002456"/>
        <obo:IAO_0000115>A bay on the Red Sea, off the coast of Eritrea.</obo:IAO_0000115>
        <oboInOwl:hasOBONamespace>GAZ</oboInOwl:hasOBONamespace>
        <oboInOwl:id>GAZ:00146201</oboInOwl:id>
        <rdfs:label>Amphila Bay</rdfs:label>
    </owl:NamedIndividual>
    


    <!-- http://purl.obolibrary.org/obo/GAZ_00176003 -->

    <owl:NamedIndividual rdf:about="http://purl.obolibrary.org/obo/GAZ_00176003">
        <obo:RO_0001025 rdf:resource="http://purl.obolibrary.org/obo/GAZ_00002456"/>
        <obo:IAO_0000115>A small 145 m long and 50 m wide artificial island in the Red Sea at the southern mouth of the Suez Canal.</obo:IAO_0000115>
        <oboInOwl:hasOBONamespace>GAZ</oboInOwl:hasOBONamespace>
        <oboInOwl:id>GAZ:00176003</oboInOwl:id>
        <rdfs:label>Al Jazeera Al Khadraa</rdfs:label>
    </owl:NamedIndividual>
    


    <!-- http://purl.obolibrary.org/obo/GAZ_00176004 -->

    <owl:NamedIndividual rdf:about="http://purl.obolibrary.org/obo/GAZ_00176004">
        <obo:RO_0001025 rdf:resource="http://purl.obolibrary.org/obo/GAZ_00000654"/>
        <obo:IAO_0000115>A peninsula in Egypt extending into the Red Sea. The inlet of water sheltered to the south of it is called Foul Bay, at the head of which sits the ancient port of Berenice.</obo:IAO_0000115>
        <oboInOwl:hasOBONamespace>GAZ</oboInOwl:hasOBONamespace>
        <oboInOwl:id>GAZ:00176004</oboInOwl:id>
        <rdfs:label>Ras Banas</rdfs:label>
    </owl:NamedIndividual>
    


    <!-- http://purl.obolibrary.org/obo/GAZ_00176005 -->

    <owl:NamedIndividual rdf:about="http://purl.obolibrary.org/obo/GAZ_00176005">
        <obo:RO_0001025 rdf:resource="http://purl.obolibrary.org/obo/GAZ_00000670"/>
        <obo:RO_0001025 rdf:resource="http://purl.obolibrary.org/obo/GAZ_00007862"/>
        <obo:IAO_0000115>An island in the northern Gulf of Aqaba off the shore of Egypt&apos;s eastern Sinai Peninsula.</obo:IAO_0000115>
        <oboInOwl:hasOBONamespace>GAZ</oboInOwl:hasOBONamespace>
        <oboInOwl:id>GAZ:00176005</oboInOwl:id>
        <rdfs:label>Pharaoh&apos;s Island</rdfs:label>
    </owl:NamedIndividual>
    


    <!-- http://purl.obolibrary.org/obo/GAZ_00176006 -->

    <owl:NamedIndividual rdf:about="http://purl.obolibrary.org/obo/GAZ_00176006">
        <obo:RO_0001025 rdf:resource="http://purl.obolibrary.org/obo/GAZ_00002456"/>
        <obo:IAO_0000115>An island off the coast of Saudi Arabia.</obo:IAO_0000115>
        <oboInOwl:hasOBONamespace>GAZ</oboInOwl:hasOBONamespace>
        <oboInOwl:id>GAZ:00176006</oboInOwl:id>
        <rdfs:label>Saso Island</rdfs:label>
    </owl:NamedIndividual>
    


    <!-- http://purl.obolibrary.org/obo/GAZ_00193804 -->

    <owl:NamedIndividual rdf:about="http://purl.obolibrary.org/obo/GAZ_00193804">
        <obo:RO_0001025 rdf:resource="http://purl.obolibrary.org/obo/GAZ_00007862"/>
        <obo:IAO_0000115>A protected area located on the Red Sea south of Eilat.</obo:IAO_0000115>
        <oboInOwl:hasOBONamespace>GAZ</oboInOwl:hasOBONamespace>
        <oboInOwl:id>GAZ:00193804</oboInOwl:id>
        <rdfs:label>Coral Beach Nature Reserve</rdfs:label>
    </owl:NamedIndividual>
    


    <!-- http://purl.obolibrary.org/obo/GAZ_00193938 -->

    <owl:NamedIndividual rdf:about="http://purl.obolibrary.org/obo/GAZ_00193938">
        <obo:RO_0001025 rdf:resource="http://purl.obolibrary.org/obo/GAZ_00000670"/>
        <obo:IAO_0000115>A saline desert lake located on the edge of the Red Sea, about 18 km south of Eilat in the Sinai Peninsula, Israel, very close to the border with Egypt.</obo:IAO_0000115>
        <oboInOwl:hasOBONamespace>GAZ</oboInOwl:hasOBONamespace>
        <oboInOwl:id>GAZ:00193938</oboInOwl:id>
        <rdfs:label>Solar Lake</rdfs:label>
    </owl:NamedIndividual>
    


    <!-- http://purl.obolibrary.org/obo/GAZ_00230302 -->

    <owl:NamedIndividual rdf:about="http://purl.obolibrary.org/obo/GAZ_00230302">
        <obo:RO_0001025 rdf:resource="http://purl.obolibrary.org/obo/GAZ_00009949"/>
        <obo:IAO_0000115>An irrigation canal. Cosntructed 1873.</obo:IAO_0000115>
        <oboInOwl:hasOBONamespace>GAZ</oboInOwl:hasOBONamespace>
        <oboInOwl:id>GAZ:00230302</oboInOwl:id>
        <rdfs:label>Ibrahimiya Canal</rdfs:label>
    </owl:NamedIndividual>
    


    <!-- http://purl.obolibrary.org/obo/GAZ_00230304 -->

    <owl:NamedIndividual rdf:about="http://purl.obolibrary.org/obo/GAZ_00230304"/>
    


    <!-- http://purl.obolibrary.org/obo/GAZ_00230305 -->

    <owl:NamedIndividual rdf:about="http://purl.obolibrary.org/obo/GAZ_00230305"/>
    


    <!-- http://purl.obolibrary.org/obo/GAZ_00230306 -->

    <owl:NamedIndividual rdf:about="http://purl.obolibrary.org/obo/GAZ_00230306">
        <obo:RO_0001025 rdf:resource="http://purl.obolibrary.org/obo/GAZ_00230307"/>
        <obo:IAO_0000115>A mountain range in the area of the Egyptian-Libyan-Sudanese border.</obo:IAO_0000115>
        <oboInOwl:hasOBONamespace>GAZ</oboInOwl:hasOBONamespace>
        <oboInOwl:id>GAZ:00230306</oboInOwl:id>
        <rdfs:label>Jebel Uweinat</rdfs:label>
    </owl:NamedIndividual>
    


    <!-- http://purl.obolibrary.org/obo/GAZ_00230307 -->

    <owl:NamedIndividual rdf:about="http://purl.obolibrary.org/obo/GAZ_00230307">
        <obo:IAO_0000115>A plateau in the remote southwest corner of Egypt.</obo:IAO_0000115>
        <oboInOwl:hasOBONamespace>GAZ</oboInOwl:hasOBONamespace>
        <oboInOwl:id>GAZ:00230307</oboInOwl:id>
        <rdfs:label>Gilf Kebir</rdfs:label>
    </owl:NamedIndividual>
    


    <!-- http://purl.obolibrary.org/obo/GAZ_00230308 -->

    <owl:NamedIndividual rdf:about="http://purl.obolibrary.org/obo/GAZ_00230308">
        <obo:RO_0001025 rdf:resource="http://purl.obolibrary.org/obo/GAZ_00230307"/>
        <obo:IAO_0000115>An impact crater.</obo:IAO_0000115>
        <oboInOwl:hasOBONamespace>GAZ</oboInOwl:hasOBONamespace>
        <oboInOwl:id>GAZ:00230308</oboInOwl:id>
        <rdfs:label>Kebira Crater</rdfs:label>
    </owl:NamedIndividual>
    


    <!-- http://purl.obolibrary.org/obo/GAZ_00230309 -->

    <owl:NamedIndividual rdf:about="http://purl.obolibrary.org/obo/GAZ_00230309">
        <obo:RO_0001025 rdf:resource="http://purl.obolibrary.org/obo/GAZ_00230307"/>
        <obo:IAO_0000115>A dry river bed.</obo:IAO_0000115>
        <oboInOwl:hasOBONamespace>GAZ</oboInOwl:hasOBONamespace>
        <oboInOwl:id>GAZ:00230309</oboInOwl:id>
        <rdfs:label>Wadi Akhdar</rdfs:label>
    </owl:NamedIndividual>
    


    <!-- http://purl.obolibrary.org/obo/GAZ_00230310 -->

    <owl:NamedIndividual rdf:about="http://purl.obolibrary.org/obo/GAZ_00230310">
        <obo:RO_0001025 rdf:resource="http://purl.obolibrary.org/obo/GAZ_00230307"/>
        <obo:IAO_0000115>A dry river bed.</obo:IAO_0000115>
        <oboInOwl:hasOBONamespace>GAZ</oboInOwl:hasOBONamespace>
        <oboInOwl:id>GAZ:00230310</oboInOwl:id>
        <rdfs:label>Wadi Bakht</rdfs:label>
    </owl:NamedIndividual>
    


    <!-- http://purl.obolibrary.org/obo/GAZ_00230311 -->

    <owl:NamedIndividual rdf:about="http://purl.obolibrary.org/obo/GAZ_00230311">
        <obo:RO_0001025 rdf:resource="http://purl.obolibrary.org/obo/GAZ_00230307"/>
        <obo:IAO_0000115>A dry river bed.</obo:IAO_0000115>
        <oboInOwl:hasOBONamespace>GAZ</oboInOwl:hasOBONamespace>
        <oboInOwl:id>GAZ:00230311</oboInOwl:id>
        <rdfs:label>Wadi Dayiq</rdfs:label>
    </owl:NamedIndividual>
    


    <!-- http://purl.obolibrary.org/obo/GAZ_00230312 -->

    <owl:NamedIndividual rdf:about="http://purl.obolibrary.org/obo/GAZ_00230312">
        <obo:RO_0001025 rdf:resource="http://purl.obolibrary.org/obo/GAZ_00230307"/>
        <obo:IAO_0000115>A dry river bed.</obo:IAO_0000115>
        <oboInOwl:hasOBONamespace>GAZ</oboInOwl:hasOBONamespace>
        <oboInOwl:id>GAZ:00230312</oboInOwl:id>
        <rdfs:label>Wadi Firaq</rdfs:label>
    </owl:NamedIndividual>
    


    <!-- http://purl.obolibrary.org/obo/GAZ_00230313 -->

    <owl:NamedIndividual rdf:about="http://purl.obolibrary.org/obo/GAZ_00230313">
        <obo:RO_0001025 rdf:resource="http://purl.obolibrary.org/obo/GAZ_00230307"/>
        <obo:IAO_0000115>A dry river bed.</obo:IAO_0000115>
        <oboInOwl:hasOBONamespace>GAZ</oboInOwl:hasOBONamespace>
        <oboInOwl:id>GAZ:00230313</oboInOwl:id>
        <rdfs:label>Wadi Gazayir</rdfs:label>
    </owl:NamedIndividual>
    


    <!-- http://purl.obolibrary.org/obo/GAZ_00230314 -->

    <owl:NamedIndividual rdf:about="http://purl.obolibrary.org/obo/GAZ_00230314">
        <obo:RO_0001025 rdf:resource="http://purl.obolibrary.org/obo/GAZ_00230307"/>
        <obo:IAO_0000115>A dry river bed.</obo:IAO_0000115>
        <oboInOwl:hasOBONamespace>GAZ</oboInOwl:hasOBONamespace>
        <oboInOwl:id>GAZ:00230314</oboInOwl:id>
        <rdfs:label>Wadi Maftuh</rdfs:label>
    </owl:NamedIndividual>
    


    <!-- http://purl.obolibrary.org/obo/GAZ_00230315 -->

    <owl:NamedIndividual rdf:about="http://purl.obolibrary.org/obo/GAZ_00230315">
        <obo:RO_0001025 rdf:resource="http://purl.obolibrary.org/obo/GAZ_00230307"/>
        <obo:IAO_0000115>A dry river bed.</obo:IAO_0000115>
        <oboInOwl:hasOBONamespace>GAZ</oboInOwl:hasOBONamespace>
        <oboInOwl:id>GAZ:00230315</oboInOwl:id>
        <rdfs:label>Wadi Mashi</rdfs:label>
    </owl:NamedIndividual>
    


    <!-- http://purl.obolibrary.org/obo/GAZ_00230316 -->

    <owl:NamedIndividual rdf:about="http://purl.obolibrary.org/obo/GAZ_00230316">
        <obo:RO_0001025 rdf:resource="http://purl.obolibrary.org/obo/GAZ_00230307"/>
        <obo:IAO_0000115>A dry river bed.</obo:IAO_0000115>
        <oboInOwl:hasOBONamespace>GAZ</oboInOwl:hasOBONamespace>
        <oboInOwl:id>GAZ:00230316</oboInOwl:id>
        <rdfs:label>Wadi Sura</rdfs:label>
    </owl:NamedIndividual>
    


    <!-- http://purl.obolibrary.org/obo/GAZ_00230317 -->

    <owl:NamedIndividual rdf:about="http://purl.obolibrary.org/obo/GAZ_00230317">
        <obo:RO_0001025 rdf:resource="http://purl.obolibrary.org/obo/GAZ_00230307"/>
        <obo:IAO_0000115>A dry river bed.</obo:IAO_0000115>
        <oboInOwl:hasOBONamespace>GAZ</oboInOwl:hasOBONamespace>
        <oboInOwl:id>GAZ:00230317</oboInOwl:id>
        <rdfs:label>Wadi Wassa</rdfs:label>
    </owl:NamedIndividual>
    


    <!-- http://purl.obolibrary.org/obo/GAZ_00230318 -->

    <owl:NamedIndividual rdf:about="http://purl.obolibrary.org/obo/GAZ_00230318">
        <obo:RO_0001025 rdf:resource="http://purl.obolibrary.org/obo/GAZ_00000645"/>
        <obo:IAO_0000115>A wadi south-east of Aswan in southern Egypt. Its location is between Lake Nasser eastern shore and Aidhab on the Red Sea.</obo:IAO_0000115>
        <oboInOwl:hasOBONamespace>GAZ</oboInOwl:hasOBONamespace>
        <oboInOwl:id>GAZ:00230318</oboInOwl:id>
        <rdfs:label>Wadi Alalaqi</rdfs:label>
    </owl:NamedIndividual>
    


    <!-- http://purl.obolibrary.org/obo/GAZ_00230319 -->

    <owl:NamedIndividual rdf:about="http://purl.obolibrary.org/obo/GAZ_00230319">
        <obo:RO_0001025 rdf:resource="http://purl.obolibrary.org/obo/GAZ_00007521"/>
        <obo:IAO_0000115>A valley. Located in an area of undulating sand with sparse scrub vegetation 47 km west of the Nile Delta, but there are hard packed gravel soils along the northern wadi margin. The lowest part of the Wadi is a depression below sea level, 50 km long and up to 8.5 km wide, oriented NW-SE, which contains a string of small saline lakes surrounded by saline desert marsh vegetation.</obo:IAO_0000115>
        <oboInOwl:hasOBONamespace>GAZ</oboInOwl:hasOBONamespace>
        <oboInOwl:id>GAZ:00230319</oboInOwl:id>
        <rdfs:label>Wadi El Natrun</rdfs:label>
    </owl:NamedIndividual>
    


    <!-- http://purl.obolibrary.org/obo/GAZ_00230320 -->

    <owl:NamedIndividual rdf:about="http://purl.obolibrary.org/obo/GAZ_00230320">
        <obo:RO_0001025 rdf:resource="http://purl.obolibrary.org/obo/GAZ_00066400"/>
        <obo:IAO_0000115>A valley in Egypt where, for a period of nearly 500 years from the 16th to 11th century BC, tombs were constructed for the kings and powerful nobles of the New Kingdom (the Eighteenth to the Twentieth Dynasties of Ancient Egypt). The valley stands on the west bank of the Nile, opposite Thebes (modern Luxor), within the heart of the Theban Necropolis. The wadi consists of two valleys, East Valley (where the majority of the royal tombs situated) and West Valley.</obo:IAO_0000115>
        <oboInOwl:hasOBONamespace>GAZ</oboInOwl:hasOBONamespace>
        <oboInOwl:id>GAZ:00230320</oboInOwl:id>
        <rdfs:label>Wadi Biban el-Muluk</rdfs:label>
    </owl:NamedIndividual>
    


    <!-- http://purl.obolibrary.org/obo/GAZ_00230321 -->

    <owl:NamedIndividual rdf:about="http://purl.obolibrary.org/obo/GAZ_00230321">
        <obo:RO_0001025 rdf:resource="http://purl.obolibrary.org/obo/GAZ_00000666"/>
        <obo:IAO_0000115>Hot springs. They originate at Gebel Ataka, the northern most mountain in the Eastern Desert.</obo:IAO_0000115>
        <oboInOwl:hasOBONamespace>GAZ</oboInOwl:hasOBONamespace>
        <oboInOwl:id>GAZ:00230321</oboInOwl:id>
        <rdfs:label>Ain Sukhna</rdfs:label>
    </owl:NamedIndividual>
    


    <!-- http://purl.obolibrary.org/obo/GAZ_00230322 -->

    <owl:NamedIndividual rdf:about="http://purl.obolibrary.org/obo/GAZ_00230322">
        <obo:RO_0001025 rdf:resource="http://purl.obolibrary.org/obo/GAZ_00000670"/>
        <obo:IAO_0000115>An oasis valley in the southern Sinai region of Egypt.</obo:IAO_0000115>
        <oboInOwl:hasOBONamespace>GAZ</oboInOwl:hasOBONamespace>
        <oboInOwl:id>GAZ:00230322</oboInOwl:id>
        <rdfs:label>Wadi Faran</rdfs:label>
    </owl:NamedIndividual>
    


    <!-- http://purl.obolibrary.org/obo/GAZ_00230323 -->

    <owl:NamedIndividual rdf:about="http://purl.obolibrary.org/obo/GAZ_00230323">
        <obo:RO_0001025 rdf:resource="http://purl.obolibrary.org/obo/GAZ_00230307"/>
        <obo:IAO_0000115>A cave in southwest Egypt, near the border with Libya, in the mountainous Gilf Kebir region of the Sahara Desert.</obo:IAO_0000115>
        <oboInOwl:hasOBONamespace>GAZ</oboInOwl:hasOBONamespace>
        <oboInOwl:id>GAZ:00230323</oboInOwl:id>
        <rdfs:label>Cave of Swimmers</rdfs:label>
    </owl:NamedIndividual>
    


    <!-- http://purl.obolibrary.org/obo/GAZ_00230324 -->

    <owl:NamedIndividual rdf:about="http://purl.obolibrary.org/obo/GAZ_00230324">
        <obo:RO_0001025 rdf:resource="http://purl.obolibrary.org/obo/GAZ_00058890"/>
        <obo:IAO_0000115>An island in the first cataract of the Nile River, Egypt.</obo:IAO_0000115>
        <oboInOwl:hasOBONamespace>GAZ</oboInOwl:hasOBONamespace>
        <oboInOwl:id>GAZ:00230324</oboInOwl:id>
        <rdfs:label>Bigeh</rdfs:label>
    </owl:NamedIndividual>
    


    <!-- http://purl.obolibrary.org/obo/GAZ_00230325 -->

    <owl:NamedIndividual rdf:about="http://purl.obolibrary.org/obo/GAZ_00230325">
        <obo:RO_0001025 rdf:resource="http://purl.obolibrary.org/obo/GAZ_00000645"/>
        <obo:IAO_0000115>An island in the River Nile, located just downstream of the First Cataract.</obo:IAO_0000115>
        <oboInOwl:hasOBONamespace>GAZ</oboInOwl:hasOBONamespace>
        <oboInOwl:id>GAZ:00230325</oboInOwl:id>
        <rdfs:label>Elephantine</rdfs:label>
    </owl:NamedIndividual>
    


    <!-- http://purl.obolibrary.org/obo/GAZ_00230326 -->

    <owl:NamedIndividual rdf:about="http://purl.obolibrary.org/obo/GAZ_00230326">
        <obo:RO_0001025 rdf:resource="http://purl.obolibrary.org/obo/GAZ_00005648"/>
        <obo:IAO_0000115>An island located in the Nile River, in central Cairo.</obo:IAO_0000115>
        <oboInOwl:hasOBONamespace>GAZ</oboInOwl:hasOBONamespace>
        <oboInOwl:id>GAZ:00230326</oboInOwl:id>
        <rdfs:label>Gezira Island</rdfs:label>
    </owl:NamedIndividual>
    


    <!-- http://purl.obolibrary.org/obo/GAZ_00230327 -->

    <owl:NamedIndividual rdf:about="http://purl.obolibrary.org/obo/GAZ_00230327">
        <obo:RO_0001025 rdf:resource="http://purl.obolibrary.org/obo/GAZ_00000645"/>
        <obo:IAO_0000115>An oval-shaped island in the Nile at Aswan, Egypt.</obo:IAO_0000115>
        <oboInOwl:hasOBONamespace>GAZ</oboInOwl:hasOBONamespace>
        <oboInOwl:id>GAZ:00230327</oboInOwl:id>
        <rdfs:label>Geziret an-Nabatat</rdfs:label>
    </owl:NamedIndividual>
    


    <!-- http://purl.obolibrary.org/obo/GAZ_00230398 -->

    <owl:NamedIndividual rdf:about="http://purl.obolibrary.org/obo/GAZ_00230398">
        <obo:IAO_0000115>A river. A tributary of the Jamma River. Along with the Adabay River, it defined the border of the former district of Marra Biete.</obo:IAO_0000115>
        <oboInOwl:hasOBONamespace>GAZ</oboInOwl:hasOBONamespace>
        <oboInOwl:id>GAZ:00230398</oboInOwl:id>
        <rdfs:label>Wanchet River</rdfs:label>
    </owl:NamedIndividual>
    


    <!-- http://purl.obolibrary.org/obo/GAZ_00230400 -->

    <owl:NamedIndividual rdf:about="http://purl.obolibrary.org/obo/GAZ_00230400">
        <obo:IAO_0000115>A river in Sudan, Africa. The most southerly of the great eastern tributaries of the Nile, the Sobat enters the White Nile at Dolieb Hill, near the city of Malakal in the Upper Nile state of Sudan.</obo:IAO_0000115>
        <oboInOwl:hasOBONamespace>GAZ</oboInOwl:hasOBONamespace>
        <oboInOwl:id>GAZ:00230400</oboInOwl:id>
        <rdfs:label>Sobat River</rdfs:label>
    </owl:NamedIndividual>
    


    <!-- http://purl.obolibrary.org/obo/GAZ_00230410 -->

    <owl:NamedIndividual rdf:about="http://purl.obolibrary.org/obo/GAZ_00230410">
        <obo:IAO_0000115>A river of southwestern Ethiopia. It is a tributary of the Baro River.</obo:IAO_0000115>
        <oboInOwl:hasOBONamespace>GAZ</oboInOwl:hasOBONamespace>
        <oboInOwl:id>GAZ:00230410</oboInOwl:id>
        <rdfs:label>Jikawo River</rdfs:label>
    </owl:NamedIndividual>
    


    <!-- http://purl.obolibrary.org/obo/GAZ_00230416 -->

    <owl:NamedIndividual rdf:about="http://purl.obolibrary.org/obo/GAZ_00230416">
        <obo:IAO_0000115>A dam. Constructed 1986.</obo:IAO_0000115>
        <oboInOwl:hasOBONamespace>GAZ</oboInOwl:hasOBONamespace>
        <oboInOwl:id>GAZ:00230416</oboInOwl:id>
        <rdfs:label>Angereb Dam</rdfs:label>
    </owl:NamedIndividual>
    


    <!-- http://purl.obolibrary.org/obo/GAZ_00230530 -->

    <owl:NamedIndividual rdf:about="http://purl.obolibrary.org/obo/GAZ_00230530">
        <obo:IAO_0000115>A valley in west-central Libya, arising out of the Sawda Mountains, situated between the towns Wanzarik and Umm al-&apos;Abid in the west and east, respectively.</obo:IAO_0000115>
        <oboInOwl:hasOBONamespace>GAZ</oboInOwl:hasOBONamespace>
        <oboInOwl:id>GAZ:00230530</oboInOwl:id>
        <rdfs:label>Wadi ash-Shati&apos;</rdfs:label>
    </owl:NamedIndividual>
    


    <!-- http://purl.obolibrary.org/obo/GAZ_00230531 -->

    <owl:NamedIndividual rdf:about="http://purl.obolibrary.org/obo/GAZ_00230531">
        <obo:IAO_0000115>A primarily erg desert in southwestern Libya and is considered part of the Sahara desert complex, although it is separated from the southern Sahara by the Tibesti Mountains and the Tassili n&apos;Ajjer.</obo:IAO_0000115>
        <oboInOwl:hasOBONamespace>GAZ</oboInOwl:hasOBONamespace>
        <oboInOwl:id>GAZ:00230531</oboInOwl:id>
        <rdfs:label>Murzuq Desert</rdfs:label>
    </owl:NamedIndividual>
    


    <!-- http://purl.obolibrary.org/obo/GAZ_00230545 -->

    <owl:NamedIndividual rdf:about="http://purl.obolibrary.org/obo/GAZ_00230545">
        <obo:IAO_0000115>An erg located in the far south-east of Western Sahara.</obo:IAO_0000115>
        <oboInOwl:hasOBONamespace>GAZ</oboInOwl:hasOBONamespace>
        <oboInOwl:id>GAZ:00230545</oboInOwl:id>
        <rdfs:label>Zug</rdfs:label>
    </owl:NamedIndividual>
    


    <!-- http://purl.obolibrary.org/obo/GAZ_00230712 -->

    <owl:NamedIndividual rdf:about="http://purl.obolibrary.org/obo/GAZ_00230712">
        <obo:IAO_0000115>A sandstone massif in Mali&apos;s Kidal Region.</obo:IAO_0000115>
        <oboInOwl:hasOBONamespace>GAZ</oboInOwl:hasOBONamespace>
        <oboInOwl:id>GAZ:00230712</oboInOwl:id>
        <rdfs:label>Adrar des Ifoghas</rdfs:label>
    </owl:NamedIndividual>
    


    <!-- http://purl.obolibrary.org/obo/GAZ_00231580 -->

    <owl:NamedIndividual rdf:about="http://purl.obolibrary.org/obo/GAZ_00231580">
        <obo:IAO_0000115>A plateau that lies in eastern Mauritania, forming a stony part of the Sahara Desert.</obo:IAO_0000115>
        <oboInOwl:hasOBONamespace>GAZ</oboInOwl:hasOBONamespace>
        <oboInOwl:id>GAZ:00231580</oboInOwl:id>
        <rdfs:label>Tagant Plateau</rdfs:label>
    </owl:NamedIndividual>
    


    <!-- http://purl.obolibrary.org/obo/GAZ_00231625 -->

    <owl:NamedIndividual rdf:about="http://purl.obolibrary.org/obo/GAZ_00231625">
        <obo:IAO_0000115>A highland area of the Sahara Desert in northern Mauritania.</obo:IAO_0000115>
        <oboInOwl:hasOBONamespace>GAZ</oboInOwl:hasOBONamespace>
        <oboInOwl:id>GAZ:00231625</oboInOwl:id>
        <rdfs:label>Adrar Plateau</rdfs:label>
    </owl:NamedIndividual>
    


    <!-- http://purl.obolibrary.org/obo/GAZ_00233408 -->

    <owl:NamedIndividual rdf:about="http://purl.obolibrary.org/obo/GAZ_00233408">
        <obo:IAO_0000115>A protected area. Established 1988-01-01.</obo:IAO_0000115>
        <oboInOwl:hasOBONamespace>GAZ</oboInOwl:hasOBONamespace>
        <oboInOwl:id>GAZ:00233408</oboInOwl:id>
        <rdfs:label>Air and Tenere Addax Sanctuary</rdfs:label>
    </owl:NamedIndividual>
    


    <!-- http://purl.obolibrary.org/obo/GAZ_00233409 -->

    <owl:NamedIndividual rdf:about="http://purl.obolibrary.org/obo/GAZ_00233409">
        <obo:IAO_0000115>A protected area. It includes both the eastern half of the Air Mountains and the western sections of the Tenere desert.</obo:IAO_0000115>
        <oboInOwl:hasOBONamespace>GAZ</oboInOwl:hasOBONamespace>
        <oboInOwl:id>GAZ:00233409</oboInOwl:id>
        <rdfs:label>Air and Tenere National Nature Reserve</rdfs:label>
    </owl:NamedIndividual>
    


    <!-- http://purl.obolibrary.org/obo/GAZ_00233411 -->

    <owl:NamedIndividual rdf:about="http://purl.obolibrary.org/obo/GAZ_00233411">
        <obo:IAO_0000115>A plateau that ies in the Sahara, in north eastern Niger.</obo:IAO_0000115>
        <oboInOwl:hasOBONamespace>GAZ</oboInOwl:hasOBONamespace>
        <oboInOwl:id>GAZ:00233411</oboInOwl:id>
        <rdfs:label>Djado Plateau</rdfs:label>
    </owl:NamedIndividual>
    


    <!-- http://purl.obolibrary.org/obo/GAZ_00233412 -->

    <owl:NamedIndividual rdf:about="http://purl.obolibrary.org/obo/GAZ_00233412">
        <obo:RO_0001025 rdf:resource="http://purl.obolibrary.org/obo/GAZ_00103898"/>
        <obo:RO_0001025 rdf:resource="http://purl.obolibrary.org/obo/GAZ_00233408"/>
        <obo:IAO_0000115>A mountain range in Niger in the northeastern section of the Air Massif, about 100 km ENE of the town of Iferouane and 30 km NE of the Tezerik oasis. Isolated from the main Massif by dune seas of the Erg of Tenere and a flat gravely Desert pavement plain.</obo:IAO_0000115>
        <oboInOwl:hasOBONamespace>GAZ</oboInOwl:hasOBONamespace>
        <oboInOwl:id>GAZ:00233412</oboInOwl:id>
        <rdfs:label>Montagnes Bleus</rdfs:label>
    </owl:NamedIndividual>
    


    <!-- http://purl.obolibrary.org/obo/GAZ_00233432 -->

    <owl:NamedIndividual rdf:about="http://purl.obolibrary.org/obo/GAZ_00233432">
        <obo:RO_0001025 rdf:resource="http://purl.obolibrary.org/obo/GAZ_00051198"/>
        <obo:IAO_0000115>An oasis surrounded by the Tenere dessert and the dunes of the Erg of Bilma in eastern Niger, placed on the western edge of the small Agram mountain outcropping.</obo:IAO_0000115>
        <oboInOwl:hasOBONamespace>GAZ</oboInOwl:hasOBONamespace>
        <oboInOwl:id>GAZ:00233432</oboInOwl:id>
        <rdfs:label>Fachi</rdfs:label>
    </owl:NamedIndividual>
    


    <!-- http://purl.obolibrary.org/obo/GAZ_00233534 -->

    <owl:NamedIndividual rdf:about="http://purl.obolibrary.org/obo/GAZ_00233534">
        <obo:IAO_0000115>A lake. Formed by a widening of the channel of the Bahr el Ghazal.</obo:IAO_0000115>
        <oboInOwl:hasOBONamespace>GAZ</oboInOwl:hasOBONamespace>
        <oboInOwl:id>GAZ:00233534</oboInOwl:id>
        <rdfs:label>Lake Ambadi</rdfs:label>
    </owl:NamedIndividual>
    


    <!-- http://purl.obolibrary.org/obo/GAZ_00233536 -->

    <owl:NamedIndividual rdf:about="http://purl.obolibrary.org/obo/GAZ_00233536">
        <obo:IAO_0000115>A dam on the Blue Nile near the town of Sennar, Sudan. Constructed 1925.</obo:IAO_0000115>
        <oboInOwl:hasOBONamespace>GAZ</oboInOwl:hasOBONamespace>
        <oboInOwl:id>GAZ:00233536</oboInOwl:id>
        <rdfs:label>Sennar Dam</rdfs:label>
    </owl:NamedIndividual>
    


    <!-- http://purl.obolibrary.org/obo/GAZ_00233537 -->

    <owl:NamedIndividual rdf:about="http://purl.obolibrary.org/obo/GAZ_00233537">
        <obo:IAO_0000115>A hydroelectric dam. Impounds El Roseires Lake. Completed 1966.</obo:IAO_0000115>
        <oboInOwl:hasOBONamespace>GAZ</oboInOwl:hasOBONamespace>
        <oboInOwl:id>GAZ:00233537</oboInOwl:id>
        <rdfs:label>El Roseires Dam</rdfs:label>
    </owl:NamedIndividual>
    


    <!-- http://purl.obolibrary.org/obo/GAZ_00233540 -->

    <owl:NamedIndividual rdf:about="http://purl.obolibrary.org/obo/GAZ_00233540">
        <obo:IAO_0000115>An island on the White Nile to the south of Khartoum, Sudan.</obo:IAO_0000115>
        <oboInOwl:hasOBONamespace>GAZ</oboInOwl:hasOBONamespace>
        <oboInOwl:id>GAZ:00233540</oboInOwl:id>
        <rdfs:label>Aba Island</rdfs:label>
    </owl:NamedIndividual>
    


    <!-- http://purl.obolibrary.org/obo/GAZ_00233541 -->

    <owl:NamedIndividual rdf:about="http://purl.obolibrary.org/obo/GAZ_00233541">
        <obo:IAO_0000115>One of the biggest islands in the Nile and the second biggest island in Sudan. It is 56 km Northern to Dongola the capital of the Northern State in Sudan.</obo:IAO_0000115>
        <oboInOwl:hasOBONamespace>GAZ</oboInOwl:hasOBONamespace>
        <oboInOwl:id>GAZ:00233541</oboInOwl:id>
        <rdfs:label>Badien Island</rdfs:label>
    </owl:NamedIndividual>
    


    <!-- http://purl.obolibrary.org/obo/GAZ_00233542 -->

    <owl:NamedIndividual rdf:about="http://purl.obolibrary.org/obo/GAZ_00233542">
        <obo:IAO_0000115>A large island in the Nile River in Nubia between the second and third cataracts. It is 12 km long and 5.5 km wide.</obo:IAO_0000115>
        <oboInOwl:hasOBONamespace>GAZ</oboInOwl:hasOBONamespace>
        <oboInOwl:id>GAZ:00233542</oboInOwl:id>
        <rdfs:label>Sai</rdfs:label>
    </owl:NamedIndividual>
    


    <!-- http://purl.obolibrary.org/obo/GAZ_00233543 -->

    <owl:NamedIndividual rdf:about="http://purl.obolibrary.org/obo/GAZ_00233543">
        <obo:IAO_0000115>An island in Sudan where the White Nile and Blue Nile merge to form the main Nile. It is surrounded by Khartoum, Omdurman and Khartoum North.</obo:IAO_0000115>
        <oboInOwl:hasOBONamespace>GAZ</oboInOwl:hasOBONamespace>
        <oboInOwl:id>GAZ:00233543</oboInOwl:id>
        <rdfs:label>Tuti Island</rdfs:label>
    </owl:NamedIndividual>
    


    <!-- http://purl.obolibrary.org/obo/GAZ_00233583 -->

    <owl:NamedIndividual rdf:about="http://purl.obolibrary.org/obo/GAZ_00233583">
        <oboInOwl:hasOBONamespace>GAZ</oboInOwl:hasOBONamespace>
        <oboInOwl:id>GAZ:00233583</oboInOwl:id>
        <rdfs:label>Schott Dscherid</rdfs:label>
    </owl:NamedIndividual>
    


    <!-- http://purl.obolibrary.org/obo/GAZ_00237174 -->

    <owl:NamedIndividual rdf:about="http://purl.obolibrary.org/obo/GAZ_00237174">
        <obo:IAO_0000115>A hydroelectric power station across the White Nile near to its source at Lake Victoria in Uganda.</obo:IAO_0000115>
        <oboInOwl:hasOBONamespace>GAZ</oboInOwl:hasOBONamespace>
        <oboInOwl:id>GAZ:00237174</oboInOwl:id>
        <rdfs:label>Nalubaale Power Station</rdfs:label>
    </owl:NamedIndividual>
    


    <!-- http://purl.obolibrary.org/obo/GAZ_00237175 -->

    <owl:NamedIndividual rdf:about="http://purl.obolibrary.org/obo/GAZ_00237175">
        <obo:IAO_0000115>A hydroelectric power station located in Jinja, Jinja District, in eastern central Uganda.</obo:IAO_0000115>
        <oboInOwl:hasOBONamespace>GAZ</oboInOwl:hasOBONamespace>
        <oboInOwl:id>GAZ:00237175</oboInOwl:id>
        <rdfs:label>Kiira Power Station</rdfs:label>
    </owl:NamedIndividual>
    


    <!-- http://purl.obolibrary.org/obo/GAZ_00237176 -->

    <owl:NamedIndividual rdf:about="http://purl.obolibrary.org/obo/GAZ_00237176">
        <obo:IAO_0000115>A hydroelectric power project located at the headwaters of River Nile, about 16 km north of Jinja at the former location of Bujagali Falls.</obo:IAO_0000115>
        <oboInOwl:hasOBONamespace>GAZ</oboInOwl:hasOBONamespace>
        <oboInOwl:id>GAZ:00237176</oboInOwl:id>
        <rdfs:label>Bujagali Power Station</rdfs:label>
    </owl:NamedIndividual>
    


    <!-- http://purl.obolibrary.org/obo/GAZ_00237412 -->

    <owl:NamedIndividual rdf:about="http://purl.obolibrary.org/obo/GAZ_00237412">
        <obo:IAO_0000115>A river of eastern Uganda in eastern Africa. It flows in a southern and south-westerly direction and eventually via the Okere River reaches Lake Kyoga.</obo:IAO_0000115>
        <oboInOwl:hasOBONamespace>GAZ</oboInOwl:hasOBONamespace>
        <oboInOwl:id>GAZ:00237412</oboInOwl:id>
        <rdfs:label>Okot River</rdfs:label>
    </owl:NamedIndividual>
    


    <!-- http://purl.obolibrary.org/obo/GAZ_00241987 -->

    <owl:NamedIndividual rdf:about="http://purl.obolibrary.org/obo/GAZ_00241987">
        <obo:RO_0001025 rdf:resource="http://purl.obolibrary.org/obo/GAZ_00000654"/>
        <obo:IAO_0000115>An administrative region (kism) of Red Sea Governorate.</obo:IAO_0000115>
        <oboInOwl:hasOBONamespace>GAZ</oboInOwl:hasOBONamespace>
        <oboInOwl:id>GAZ:00241987</oboInOwl:id>
        <rdfs:label>Kism El Shalateen</rdfs:label>
    </owl:NamedIndividual>
    


    <!-- http://purl.obolibrary.org/obo/GAZ_00241988 -->

    <owl:NamedIndividual rdf:about="http://purl.obolibrary.org/obo/GAZ_00241988">
        <obo:RO_0001025 rdf:resource="http://purl.obolibrary.org/obo/GAZ_00000654"/>
        <obo:IAO_0000115>An administrative region (kism) of Red Sea Governorate.</obo:IAO_0000115>
        <oboInOwl:hasOBONamespace>GAZ</oboInOwl:hasOBONamespace>
        <oboInOwl:id>GAZ:00241988</oboInOwl:id>
        <rdfs:label>Kism Halaeeb</rdfs:label>
    </owl:NamedIndividual>
    


    <!-- http://purl.obolibrary.org/obo/GAZ_00241989 -->

    <owl:NamedIndividual rdf:about="http://purl.obolibrary.org/obo/GAZ_00241989">
        <obo:RO_0001025 rdf:resource="http://purl.obolibrary.org/obo/GAZ_00000654"/>
        <obo:IAO_0000115>An administrative region (kism) of Red Sea Governorate.</obo:IAO_0000115>
        <oboInOwl:hasOBONamespace>GAZ</oboInOwl:hasOBONamespace>
        <oboInOwl:id>GAZ:00241989</oboInOwl:id>
        <rdfs:label>Kism Marsa al &apos;Alam</rdfs:label>
    </owl:NamedIndividual>
    


    <!-- http://purl.obolibrary.org/obo/GAZ_00241990 -->

    <owl:NamedIndividual rdf:about="http://purl.obolibrary.org/obo/GAZ_00241990">
        <obo:RO_0001025 rdf:resource="http://purl.obolibrary.org/obo/GAZ_00000667"/>
        <obo:IAO_0000115>An administrative region (markaz) of Matruh Governorate.</obo:IAO_0000115>
        <oboInOwl:hasOBONamespace>GAZ</oboInOwl:hasOBONamespace>
        <oboInOwl:id>GAZ:00241990</oboInOwl:id>
        <rdfs:label>Marsa Matruh Region</rdfs:label>
    </owl:NamedIndividual>
    


    <!-- http://purl.obolibrary.org/obo/GAZ_00241991 -->

    <owl:NamedIndividual rdf:about="http://purl.obolibrary.org/obo/GAZ_00241991">
        <obo:RO_0001025 rdf:resource="http://purl.obolibrary.org/obo/GAZ_00000667"/>
        <obo:IAO_0000115>An administrative region (markaz) of Matruh Governorate.</obo:IAO_0000115>
        <oboInOwl:hasOBONamespace>GAZ</oboInOwl:hasOBONamespace>
        <oboInOwl:id>GAZ:00241991</oboInOwl:id>
        <rdfs:label>As Sallum Region</rdfs:label>
    </owl:NamedIndividual>
    


    <!-- http://purl.obolibrary.org/obo/GAZ_00241992 -->

    <owl:NamedIndividual rdf:about="http://purl.obolibrary.org/obo/GAZ_00241992">
        <obo:RO_0001025 rdf:resource="http://purl.obolibrary.org/obo/GAZ_00066423"/>
        <obo:IAO_0000115>An administrative region (kism) of North Sinai Governorate.</obo:IAO_0000115>
        <oboInOwl:hasOBONamespace>GAZ</oboInOwl:hasOBONamespace>
        <oboInOwl:id>GAZ:00241992</oboInOwl:id>
        <rdfs:label>Kism Al &apos;Arish First</rdfs:label>
    </owl:NamedIndividual>
    


    <!-- http://purl.obolibrary.org/obo/GAZ_00241993 -->

    <owl:NamedIndividual rdf:about="http://purl.obolibrary.org/obo/GAZ_00241993">
        <obo:RO_0001025 rdf:resource="http://purl.obolibrary.org/obo/GAZ_00066423"/>
        <obo:IAO_0000115>An administrative region (kism) of North Sinai Governorate.</obo:IAO_0000115>
        <oboInOwl:hasOBONamespace>GAZ</oboInOwl:hasOBONamespace>
        <oboInOwl:id>GAZ:00241993</oboInOwl:id>
        <rdfs:label>Kism Al &apos;Arish Second</rdfs:label>
    </owl:NamedIndividual>
    


    <!-- http://purl.obolibrary.org/obo/GAZ_00241994 -->

    <owl:NamedIndividual rdf:about="http://purl.obolibrary.org/obo/GAZ_00241994">
        <obo:RO_0001025 rdf:resource="http://purl.obolibrary.org/obo/GAZ_00066423"/>
        <obo:IAO_0000115>An administrative region (kism) of North Sinai Governorate.</obo:IAO_0000115>
        <oboInOwl:hasOBONamespace>GAZ</oboInOwl:hasOBONamespace>
        <oboInOwl:id>GAZ:00241994</oboInOwl:id>
        <rdfs:label>Kism Al &apos;Arish Third</rdfs:label>
    </owl:NamedIndividual>
    


    <!-- http://purl.obolibrary.org/obo/GAZ_00241995 -->

    <owl:NamedIndividual rdf:about="http://purl.obolibrary.org/obo/GAZ_00241995">
        <obo:RO_0001025 rdf:resource="http://purl.obolibrary.org/obo/GAZ_00066423"/>
        <obo:IAO_0000115>An administrative region (kism) of North Sinai Governorate.</obo:IAO_0000115>
        <oboInOwl:hasOBONamespace>GAZ</oboInOwl:hasOBONamespace>
        <oboInOwl:id>GAZ:00241995</oboInOwl:id>
        <rdfs:label>Kism Al &apos;Arish Fourth</rdfs:label>
    </owl:NamedIndividual>
    


    <!-- http://purl.obolibrary.org/obo/GAZ_00241996 -->

    <owl:NamedIndividual rdf:about="http://purl.obolibrary.org/obo/GAZ_00241996">
        <obo:RO_0001025 rdf:resource="http://purl.obolibrary.org/obo/GAZ_00000669"/>
        <obo:IAO_0000115>An administrative region (markaz) of North Sinai Governorate.</obo:IAO_0000115>
        <oboInOwl:hasOBONamespace>GAZ</oboInOwl:hasOBONamespace>
        <oboInOwl:id>GAZ:00241996</oboInOwl:id>
        <rdfs:label>Al Qusaymah Region</rdfs:label>
    </owl:NamedIndividual>
    


    <!-- http://purl.obolibrary.org/obo/GAZ_00241997 -->

    <owl:NamedIndividual rdf:about="http://purl.obolibrary.org/obo/GAZ_00241997">
        <obo:RO_0001025 rdf:resource="http://purl.obolibrary.org/obo/GAZ_00000669"/>
        <obo:IAO_0000115>An administrative region of North Sinai Governorate.</obo:IAO_0000115>
        <oboInOwl:hasOBONamespace>GAZ</oboInOwl:hasOBONamespace>
        <oboInOwl:id>GAZ:00241997</oboInOwl:id>
        <rdfs:label>Rmana Police Center</rdfs:label>
    </owl:NamedIndividual>
    


    <!-- http://purl.obolibrary.org/obo/GAZ_00241998 -->

    <owl:NamedIndividual rdf:about="http://purl.obolibrary.org/obo/GAZ_00241998">
        <obo:RO_0001025 rdf:resource="http://purl.obolibrary.org/obo/GAZ_00000668"/>
        <obo:IAO_0000115>An administrative region ) of New Valley Governorate.</obo:IAO_0000115>
        <oboInOwl:hasOBONamespace>GAZ</oboInOwl:hasOBONamespace>
        <oboInOwl:id>GAZ:00241998</oboInOwl:id>
        <rdfs:label>Paris Police Center Station</rdfs:label>
    </owl:NamedIndividual>
    


    <!-- http://purl.obolibrary.org/obo/GAZ_00241999 -->

    <owl:NamedIndividual rdf:about="http://purl.obolibrary.org/obo/GAZ_00241999">
        <obo:RO_0001025 rdf:resource="http://purl.obolibrary.org/obo/GAZ_00000655"/>
        <obo:IAO_0000115>An administrative region (kism) of Beheira Governorate.</obo:IAO_0000115>
        <oboInOwl:hasOBONamespace>GAZ</oboInOwl:hasOBONamespace>
        <oboInOwl:id>GAZ:00241999</oboInOwl:id>
        <rdfs:label>Kism West Nubariyah</rdfs:label>
    </owl:NamedIndividual>
    


    <!-- http://purl.obolibrary.org/obo/GAZ_00242000 -->

    <owl:NamedIndividual rdf:about="http://purl.obolibrary.org/obo/GAZ_00242000">
        <obo:RO_0001025 rdf:resource="http://purl.obolibrary.org/obo/GAZ_00000655"/>
        <obo:IAO_0000115>An administrative region (kism) of Beheira Governorate.</obo:IAO_0000115>
        <oboInOwl:hasOBONamespace>GAZ</oboInOwl:hasOBONamespace>
        <oboInOwl:id>GAZ:00242000</oboInOwl:id>
        <rdfs:label>Kism Kafr ad Dawwar</rdfs:label>
    </owl:NamedIndividual>
    


    <!-- http://purl.obolibrary.org/obo/GAZ_00242001 -->

    <owl:NamedIndividual rdf:about="http://purl.obolibrary.org/obo/GAZ_00242001">
        <obo:RO_0001025 rdf:resource="http://purl.obolibrary.org/obo/GAZ_00000655"/>
        <obo:IAO_0000115>An administrative region (markuz) of Beheira Governorate.</obo:IAO_0000115>
        <oboInOwl:hasOBONamespace>GAZ</oboInOwl:hasOBONamespace>
        <oboInOwl:id>GAZ:00242001</oboInOwl:id>
        <rdfs:label>Badr Region</rdfs:label>
    </owl:NamedIndividual>
    


    <!-- http://purl.obolibrary.org/obo/GAZ_00242002 -->

    <owl:NamedIndividual rdf:about="http://purl.obolibrary.org/obo/GAZ_00242002">
        <obo:RO_0001025 rdf:resource="http://purl.obolibrary.org/obo/GAZ_00000655"/>
        <obo:IAO_0000115>An administrative region of Beheira Governorate.</obo:IAO_0000115>
        <oboInOwl:hasOBONamespace>GAZ</oboInOwl:hasOBONamespace>
        <oboInOwl:id>GAZ:00242002</oboInOwl:id>
        <rdfs:label>Damanhur Station</rdfs:label>
    </owl:NamedIndividual>
    


    <!-- http://purl.obolibrary.org/obo/GAZ_00242003 -->

    <owl:NamedIndividual rdf:about="http://purl.obolibrary.org/obo/GAZ_00242003">
        <obo:RO_0001025 rdf:resource="http://purl.obolibrary.org/obo/GAZ_00030901"/>
        <obo:IAO_0000115>An administrative region (kism) of Dakahlia Governorate.</obo:IAO_0000115>
        <oboInOwl:hasOBONamespace>GAZ</oboInOwl:hasOBONamespace>
        <oboInOwl:id>GAZ:00242003</oboInOwl:id>
        <rdfs:label>Kism Al Mansurah First</rdfs:label>
    </owl:NamedIndividual>
    


    <!-- http://purl.obolibrary.org/obo/GAZ_00242004 -->

    <owl:NamedIndividual rdf:about="http://purl.obolibrary.org/obo/GAZ_00242004">
        <obo:RO_0001025 rdf:resource="http://purl.obolibrary.org/obo/GAZ_00030901"/>
        <obo:IAO_0000115>An administrative region (kism) of Dakahlia Governorate.</obo:IAO_0000115>
        <oboInOwl:hasOBONamespace>GAZ</oboInOwl:hasOBONamespace>
        <oboInOwl:id>GAZ:00242004</oboInOwl:id>
        <rdfs:label>Kism Al Mansurah Second</rdfs:label>
    </owl:NamedIndividual>
    


    <!-- http://purl.obolibrary.org/obo/GAZ_00242005 -->

    <owl:NamedIndividual rdf:about="http://purl.obolibrary.org/obo/GAZ_00242005">
        <obo:RO_0001025 rdf:resource="http://purl.obolibrary.org/obo/GAZ_00030913"/>
        <obo:IAO_0000115>An administrative region (kisim) of Dakahlia Governorate.</obo:IAO_0000115>
        <oboInOwl:hasOBONamespace>GAZ</oboInOwl:hasOBONamespace>
        <oboInOwl:id>GAZ:00242005</oboInOwl:id>
        <rdfs:label>Kism Mit Ghamr</rdfs:label>
    </owl:NamedIndividual>
    


    <!-- http://purl.obolibrary.org/obo/GAZ_00242006 -->

    <owl:NamedIndividual rdf:about="http://purl.obolibrary.org/obo/GAZ_00242006">
        <obo:RO_0001025 rdf:resource="http://purl.obolibrary.org/obo/GAZ_00000657"/>
        <obo:IAO_0000115>An administrative region (kism) of Damietta Governorate.</obo:IAO_0000115>
        <oboInOwl:hasOBONamespace>GAZ</oboInOwl:hasOBONamespace>
        <oboInOwl:id>GAZ:00242006</oboInOwl:id>
        <rdfs:label>Kism Dumyat First</rdfs:label>
    </owl:NamedIndividual>
    


    <!-- http://purl.obolibrary.org/obo/GAZ_00242007 -->

    <owl:NamedIndividual rdf:about="http://purl.obolibrary.org/obo/GAZ_00242007">
        <obo:RO_0001025 rdf:resource="http://purl.obolibrary.org/obo/GAZ_00030917"/>
        <obo:IAO_0000115>An administrative region (kism) of Damietta Governorate.</obo:IAO_0000115>
        <oboInOwl:hasOBONamespace>GAZ</oboInOwl:hasOBONamespace>
        <oboInOwl:id>GAZ:00242007</oboInOwl:id>
        <rdfs:label>Kism Dumyat Second</rdfs:label>
    </owl:NamedIndividual>
    


    <!-- http://purl.obolibrary.org/obo/GAZ_00242008 -->

    <owl:NamedIndividual rdf:about="http://purl.obolibrary.org/obo/GAZ_00242008">
        <obo:RO_0001025 rdf:resource="http://purl.obolibrary.org/obo/GAZ_00000657"/>
        <obo:IAO_0000115>An administrative region (kism) of Damietta Governorate.</obo:IAO_0000115>
        <oboInOwl:hasOBONamespace>GAZ</oboInOwl:hasOBONamespace>
        <oboInOwl:id>GAZ:00242008</oboInOwl:id>
        <rdfs:label>Kism New Dumyat City</rdfs:label>
    </owl:NamedIndividual>
    


    <!-- http://purl.obolibrary.org/obo/GAZ_00242009 -->

    <owl:NamedIndividual rdf:about="http://purl.obolibrary.org/obo/GAZ_00242009">
        <obo:RO_0001025 rdf:resource="http://purl.obolibrary.org/obo/GAZ_00000657"/>
        <obo:IAO_0000115>An administrative region (kism) of Damietta Governorate.</obo:IAO_0000115>
        <oboInOwl:hasOBONamespace>GAZ</oboInOwl:hasOBONamespace>
        <oboInOwl:id>GAZ:00242009</oboInOwl:id>
        <rdfs:label>Kism Ra&apos;s al Barr</rdfs:label>
    </owl:NamedIndividual>
    


    <!-- http://purl.obolibrary.org/obo/GAZ_00242010 -->

    <owl:NamedIndividual rdf:about="http://purl.obolibrary.org/obo/GAZ_00242010">
        <obo:RO_0001025 rdf:resource="http://purl.obolibrary.org/obo/GAZ_00066459"/>
        <obo:IAO_0000115>An administrative region (kism) of Gharbia Governorate.</obo:IAO_0000115>
        <oboInOwl:hasOBONamespace>GAZ</oboInOwl:hasOBONamespace>
        <oboInOwl:id>GAZ:00242010</oboInOwl:id>
        <rdfs:label>Kism Tanta First</rdfs:label>
    </owl:NamedIndividual>
    


    <!-- http://purl.obolibrary.org/obo/GAZ_00242011 -->

    <owl:NamedIndividual rdf:about="http://purl.obolibrary.org/obo/GAZ_00242011">
        <obo:RO_0001025 rdf:resource="http://purl.obolibrary.org/obo/GAZ_00066459"/>
        <obo:IAO_0000115>An administrative region (kism) of Gharbia Governorate.</obo:IAO_0000115>
        <oboInOwl:hasOBONamespace>GAZ</oboInOwl:hasOBONamespace>
        <oboInOwl:id>GAZ:00242011</oboInOwl:id>
        <rdfs:label>Kism Tanta Second</rdfs:label>
    </owl:NamedIndividual>
    


    <!-- http://purl.obolibrary.org/obo/GAZ_00242012 -->

    <owl:NamedIndividual rdf:about="http://purl.obolibrary.org/obo/GAZ_00242012">
        <obo:RO_0001025 rdf:resource="http://purl.obolibrary.org/obo/GAZ_00066386"/>
        <obo:IAO_0000115>An administrative region (kism) of Gharbia Governorate.</obo:IAO_0000115>
        <oboInOwl:hasOBONamespace>GAZ</oboInOwl:hasOBONamespace>
        <oboInOwl:id>GAZ:00242012</oboInOwl:id>
        <rdfs:label>Kism Al Mahallah al Kubra First</rdfs:label>
    </owl:NamedIndividual>
    


    <!-- http://purl.obolibrary.org/obo/GAZ_00242013 -->

    <owl:NamedIndividual rdf:about="http://purl.obolibrary.org/obo/GAZ_00242013">
        <obo:RO_0001025 rdf:resource="http://purl.obolibrary.org/obo/GAZ_00066386"/>
        <obo:IAO_0000115>An administrative region (kism) of Gharbia Governorate.</obo:IAO_0000115>
        <oboInOwl:hasOBONamespace>GAZ</oboInOwl:hasOBONamespace>
        <oboInOwl:id>GAZ:00242013</oboInOwl:id>
        <rdfs:label>Kism Al Mahallah al Kubra Second</rdfs:label>
    </owl:NamedIndividual>
    


    <!-- http://purl.obolibrary.org/obo/GAZ_00242014 -->

    <owl:NamedIndividual rdf:about="http://purl.obolibrary.org/obo/GAZ_00242014">
        <obo:RO_0001025 rdf:resource="http://purl.obolibrary.org/obo/GAZ_00066397"/>
        <obo:IAO_0000115>An administrative region (kism) of Ismalia Governorate.</obo:IAO_0000115>
        <oboInOwl:hasOBONamespace>GAZ</oboInOwl:hasOBONamespace>
        <oboInOwl:id>GAZ:00242014</oboInOwl:id>
        <rdfs:label>Kism Al Isma&apos;iliyah First</rdfs:label>
    </owl:NamedIndividual>
    


    <!-- http://purl.obolibrary.org/obo/GAZ_00242015 -->

    <owl:NamedIndividual rdf:about="http://purl.obolibrary.org/obo/GAZ_00242015">
        <obo:RO_0001025 rdf:resource="http://purl.obolibrary.org/obo/GAZ_00066397"/>
        <obo:IAO_0000115>An administrative region (kism) of Ismalia Governorate.</obo:IAO_0000115>
        <oboInOwl:hasOBONamespace>GAZ</oboInOwl:hasOBONamespace>
        <oboInOwl:id>GAZ:00242015</oboInOwl:id>
        <rdfs:label>Kism Al Isma&apos;iliyah Second</rdfs:label>
    </owl:NamedIndividual>
    


    <!-- http://purl.obolibrary.org/obo/GAZ_00242016 -->

    <owl:NamedIndividual rdf:about="http://purl.obolibrary.org/obo/GAZ_00242016">
        <obo:RO_0001025 rdf:resource="http://purl.obolibrary.org/obo/GAZ_00066397"/>
        <obo:IAO_0000115>An administrative region (kism) of Ismalia Governorate.</obo:IAO_0000115>
        <oboInOwl:hasOBONamespace>GAZ</oboInOwl:hasOBONamespace>
        <oboInOwl:id>GAZ:00242016</oboInOwl:id>
        <rdfs:label>Kism Al Isma&apos;iliyah Third</rdfs:label>
    </owl:NamedIndividual>
    


    <!-- http://purl.obolibrary.org/obo/GAZ_00242017 -->

    <owl:NamedIndividual rdf:about="http://purl.obolibrary.org/obo/GAZ_00242017">
        <obo:RO_0001025 rdf:resource="http://purl.obolibrary.org/obo/GAZ_00030964"/>
        <obo:IAO_0000115>An administrative region (kism) of Kafr el-Sheikh Governorate.</obo:IAO_0000115>
        <oboInOwl:hasOBONamespace>GAZ</oboInOwl:hasOBONamespace>
        <oboInOwl:id>GAZ:00242017</oboInOwl:id>
        <rdfs:label>Kism Disuq</rdfs:label>
    </owl:NamedIndividual>
    


    <!-- http://purl.obolibrary.org/obo/GAZ_00242018 -->

    <owl:NamedIndividual rdf:about="http://purl.obolibrary.org/obo/GAZ_00242018">
        <obo:RO_0001025 rdf:resource="http://purl.obolibrary.org/obo/GAZ_00030966"/>
        <obo:IAO_0000115>An administrative region (kism) of Kafr el-Sheikh Governorate.</obo:IAO_0000115>
        <oboInOwl:hasOBONamespace>GAZ</oboInOwl:hasOBONamespace>
        <oboInOwl:id>GAZ:00242018</oboInOwl:id>
        <rdfs:label>Kism Kafr ash Shaykh</rdfs:label>
    </owl:NamedIndividual>
    


    <!-- http://purl.obolibrary.org/obo/GAZ_00242019 -->

    <owl:NamedIndividual rdf:about="http://purl.obolibrary.org/obo/GAZ_00242019">
        <obo:RO_0001025 rdf:resource="http://purl.obolibrary.org/obo/GAZ_00000659"/>
        <obo:IAO_0000115>An administrative region (markaz) of Kafr el-Sheikh Governorate.</obo:IAO_0000115>
        <oboInOwl:hasOBONamespace>GAZ</oboInOwl:hasOBONamespace>
        <oboInOwl:id>GAZ:00242019</oboInOwl:id>
        <rdfs:label>Al Burullus Region</rdfs:label>
    </owl:NamedIndividual>
    


    <!-- http://purl.obolibrary.org/obo/GAZ_00242020 -->

    <owl:NamedIndividual rdf:about="http://purl.obolibrary.org/obo/GAZ_00242020">
        <obo:RO_0001025 rdf:resource="http://purl.obolibrary.org/obo/GAZ_00030919"/>
        <obo:IAO_0000115>An administrative region (kism) of Monufia Governorate.</obo:IAO_0000115>
        <oboInOwl:hasOBONamespace>GAZ</oboInOwl:hasOBONamespace>
        <oboInOwl:id>GAZ:00242020</oboInOwl:id>
        <rdfs:label>Kism Minufiyah</rdfs:label>
    </owl:NamedIndividual>
    


    <!-- http://purl.obolibrary.org/obo/GAZ_00242021 -->

    <owl:NamedIndividual rdf:about="http://purl.obolibrary.org/obo/GAZ_00242021">
        <obo:RO_0001025 rdf:resource="http://purl.obolibrary.org/obo/GAZ_00030927"/>
        <obo:IAO_0000115>An administrative region (kism) of Monufia Governorate.</obo:IAO_0000115>
        <oboInOwl:hasOBONamespace>GAZ</oboInOwl:hasOBONamespace>
        <oboInOwl:id>GAZ:00242021</oboInOwl:id>
        <rdfs:label>Kism Shibin al Kawm</rdfs:label>
    </owl:NamedIndividual>
    


    <!-- http://purl.obolibrary.org/obo/GAZ_00242022 -->

    <owl:NamedIndividual rdf:about="http://purl.obolibrary.org/obo/GAZ_00242022">
        <obo:RO_0001025 rdf:resource="http://purl.obolibrary.org/obo/GAZ_00031022"/>
        <obo:IAO_0000115>An administrative region (kism) of Qalyubia Governorate.</obo:IAO_0000115>
        <oboInOwl:hasOBONamespace>GAZ</oboInOwl:hasOBONamespace>
        <oboInOwl:id>GAZ:00242022</oboInOwl:id>
        <rdfs:label>Kism Shubra al Khaymah First</rdfs:label>
    </owl:NamedIndividual>
    


    <!-- http://purl.obolibrary.org/obo/GAZ_00242023 -->

    <owl:NamedIndividual rdf:about="http://purl.obolibrary.org/obo/GAZ_00242023">
        <obo:RO_0001025 rdf:resource="http://purl.obolibrary.org/obo/GAZ_00031022"/>
        <obo:IAO_0000115>An administrative region (kism) of Qalyubia Governorate.</obo:IAO_0000115>
        <oboInOwl:hasOBONamespace>GAZ</oboInOwl:hasOBONamespace>
        <oboInOwl:id>GAZ:00242023</oboInOwl:id>
        <rdfs:label>Kism Shubra al Khaymah Second</rdfs:label>
    </owl:NamedIndividual>
    


    <!-- http://purl.obolibrary.org/obo/GAZ_00242024 -->

    <owl:NamedIndividual rdf:about="http://purl.obolibrary.org/obo/GAZ_00242024">
        <obo:RO_0001025 rdf:resource="http://purl.obolibrary.org/obo/GAZ_00031020"/>
        <obo:IAO_0000115>An administrative region (kism) of Qalyubia Governorate.</obo:IAO_0000115>
        <oboInOwl:hasOBONamespace>GAZ</oboInOwl:hasOBONamespace>
        <oboInOwl:id>GAZ:00242024</oboInOwl:id>
        <rdfs:label>Kism Qalyub</rdfs:label>
    </owl:NamedIndividual>
    


    <!-- http://purl.obolibrary.org/obo/GAZ_00242025 -->

    <owl:NamedIndividual rdf:about="http://purl.obolibrary.org/obo/GAZ_00242025">
        <obo:RO_0001025 rdf:resource="http://purl.obolibrary.org/obo/GAZ_00031016"/>
        <obo:IAO_0000115>An administrative region (kism) of Qalyubia Governorate.</obo:IAO_0000115>
        <oboInOwl:hasOBONamespace>GAZ</oboInOwl:hasOBONamespace>
        <oboInOwl:id>GAZ:00242025</oboInOwl:id>
        <rdfs:label>Kism Banha</rdfs:label>
    </owl:NamedIndividual>
    


    <!-- http://purl.obolibrary.org/obo/GAZ_00242026 -->

    <owl:NamedIndividual rdf:about="http://purl.obolibrary.org/obo/GAZ_00242026">
        <obo:RO_0001025 rdf:resource="http://purl.obolibrary.org/obo/GAZ_00000661"/>
        <obo:IAO_0000115>An administrative region (kism) of Qalyubia Governorate.</obo:IAO_0000115>
        <oboInOwl:hasOBONamespace>GAZ</oboInOwl:hasOBONamespace>
        <oboInOwl:id>GAZ:00242026</oboInOwl:id>
        <rdfs:label>Kism Abor</rdfs:label>
    </owl:NamedIndividual>
    


    <!-- http://purl.obolibrary.org/obo/GAZ_00242027 -->

    <owl:NamedIndividual rdf:about="http://purl.obolibrary.org/obo/GAZ_00242027">
        <obo:RO_0001025 rdf:resource="http://purl.obolibrary.org/obo/GAZ_00000661"/>
        <obo:IAO_0000115>An administrative region (kism) of Qalyubia Governorate.</obo:IAO_0000115>
        <oboInOwl:hasOBONamespace>GAZ</oboInOwl:hasOBONamespace>
        <oboInOwl:id>GAZ:00242027</oboInOwl:id>
        <rdfs:label>Kism Al Khusus</rdfs:label>
    </owl:NamedIndividual>
    


    <!-- http://purl.obolibrary.org/obo/GAZ_00242028 -->

    <owl:NamedIndividual rdf:about="http://purl.obolibrary.org/obo/GAZ_00242028">
        <obo:RO_0001025 rdf:resource="http://purl.obolibrary.org/obo/GAZ_00031002"/>
        <obo:IAO_0000115>An administrative region (kism) of Sharqia Governorate.</obo:IAO_0000115>
        <oboInOwl:hasOBONamespace>GAZ</oboInOwl:hasOBONamespace>
        <oboInOwl:id>GAZ:00242028</oboInOwl:id>
        <rdfs:label>Kism Az Zaqaziq First</rdfs:label>
    </owl:NamedIndividual>
    


    <!-- http://purl.obolibrary.org/obo/GAZ_00242029 -->

    <owl:NamedIndividual rdf:about="http://purl.obolibrary.org/obo/GAZ_00242029">
        <obo:RO_0001025 rdf:resource="http://purl.obolibrary.org/obo/GAZ_00031002"/>
        <obo:IAO_0000115>An administrative region (kism) of Sharqia Governorate.</obo:IAO_0000115>
        <oboInOwl:hasOBONamespace>GAZ</oboInOwl:hasOBONamespace>
        <oboInOwl:id>GAZ:00242029</oboInOwl:id>
        <rdfs:label>Kism Az Zaqaziq Second</rdfs:label>
    </owl:NamedIndividual>
    


    <!-- http://purl.obolibrary.org/obo/GAZ_00242030 -->

    <owl:NamedIndividual rdf:about="http://purl.obolibrary.org/obo/GAZ_00242030">
        <obo:RO_0001025 rdf:resource="http://purl.obolibrary.org/obo/GAZ_00031000"/>
        <obo:IAO_0000115>An administrative region (kism) of Sharqia Governorate.</obo:IAO_0000115>
        <oboInOwl:hasOBONamespace>GAZ</oboInOwl:hasOBONamespace>
        <oboInOwl:id>GAZ:00242030</oboInOwl:id>
        <rdfs:label>Kism Faqus</rdfs:label>
    </owl:NamedIndividual>
    


    <!-- http://purl.obolibrary.org/obo/GAZ_00242031 -->

    <owl:NamedIndividual rdf:about="http://purl.obolibrary.org/obo/GAZ_00242031">
        <obo:RO_0001025 rdf:resource="http://purl.obolibrary.org/obo/GAZ_00000662"/>
        <obo:IAO_0000115>An administrative region (kism) of Sharqia Governorate.</obo:IAO_0000115>
        <oboInOwl:hasOBONamespace>GAZ</oboInOwl:hasOBONamespace>
        <oboInOwl:id>GAZ:00242031</oboInOwl:id>
        <rdfs:label>Kism Al Qurayn</rdfs:label>
    </owl:NamedIndividual>
    


    <!-- http://purl.obolibrary.org/obo/GAZ_00242032 -->

    <owl:NamedIndividual rdf:about="http://purl.obolibrary.org/obo/GAZ_00242032">
        <obo:RO_0001025 rdf:resource="http://purl.obolibrary.org/obo/GAZ_00000662"/>
        <obo:IAO_0000115>An administrative region (kism) of Sharqia Governorate.</obo:IAO_0000115>
        <oboInOwl:hasOBONamespace>GAZ</oboInOwl:hasOBONamespace>
        <oboInOwl:id>GAZ:00242032</oboInOwl:id>
        <rdfs:label>Kism As Salhiyah New</rdfs:label>
    </owl:NamedIndividual>
    


    <!-- http://purl.obolibrary.org/obo/GAZ_00242033 -->

    <owl:NamedIndividual rdf:about="http://purl.obolibrary.org/obo/GAZ_00242033">
        <obo:RO_0001025 rdf:resource="http://purl.obolibrary.org/obo/GAZ_00000662"/>
        <obo:IAO_0000115>A populated place.</obo:IAO_0000115>
        <oboInOwl:hasOBONamespace>GAZ</oboInOwl:hasOBONamespace>
        <oboInOwl:id>GAZ:00242033</oboInOwl:id>
        <rdfs:label>Madinat al &apos;Ashir min Ramadan</rdfs:label>
    </owl:NamedIndividual>
    


    <!-- http://purl.obolibrary.org/obo/GAZ_00242034 -->

    <owl:NamedIndividual rdf:about="http://purl.obolibrary.org/obo/GAZ_00242034">
        <obo:RO_0001025 rdf:resource="http://purl.obolibrary.org/obo/GAZ_00242033"/>
        <obo:IAO_0000115>An administrative region (Kism) of Sharqia Governorate.</obo:IAO_0000115>
        <oboInOwl:hasOBONamespace>GAZ</oboInOwl:hasOBONamespace>
        <oboInOwl:id>GAZ:00242034</oboInOwl:id>
        <rdfs:label>Kism 10 Ramadan City First</rdfs:label>
    </owl:NamedIndividual>
    


    <!-- http://purl.obolibrary.org/obo/GAZ_00242035 -->

    <owl:NamedIndividual rdf:about="http://purl.obolibrary.org/obo/GAZ_00242035">
        <obo:RO_0001025 rdf:resource="http://purl.obolibrary.org/obo/GAZ_00242033"/>
        <obo:IAO_0000115>An administrative region (Kism) of Sharqia Governorate.</obo:IAO_0000115>
        <oboInOwl:hasOBONamespace>GAZ</oboInOwl:hasOBONamespace>
        <oboInOwl:id>GAZ:00242035</oboInOwl:id>
        <rdfs:label>Kism 10 Ramadan City Second</rdfs:label>
    </owl:NamedIndividual>
    


    <!-- http://purl.obolibrary.org/obo/GAZ_00242036 -->

    <owl:NamedIndividual rdf:about="http://purl.obolibrary.org/obo/GAZ_00242036">
        <obo:RO_0001025 rdf:resource="http://purl.obolibrary.org/obo/GAZ_00230305"/>
        <obo:IAO_0000115>An administrative region (kism) of 6th of October Governorate.</obo:IAO_0000115>
        <oboInOwl:hasOBONamespace>GAZ</oboInOwl:hasOBONamespace>
        <oboInOwl:id>GAZ:00242036</oboInOwl:id>
        <rdfs:label>Kism Al Wahat al Bahariyah</rdfs:label>
    </owl:NamedIndividual>
    


    <!-- http://purl.obolibrary.org/obo/GAZ_00242037 -->

    <owl:NamedIndividual rdf:about="http://purl.obolibrary.org/obo/GAZ_00242037">
        <obo:RO_0001025 rdf:resource="http://purl.obolibrary.org/obo/GAZ_00230305"/>
        <obo:IAO_0000115>An administrative region (kism) of 6th of October Governorate.</obo:IAO_0000115>
        <oboInOwl:hasOBONamespace>GAZ</oboInOwl:hasOBONamespace>
        <oboInOwl:id>GAZ:00242037</oboInOwl:id>
        <rdfs:label>Kism Madinat Sittah Uktubar</rdfs:label>
    </owl:NamedIndividual>
    


    <!-- http://purl.obolibrary.org/obo/GAZ_00242038 -->

    <owl:NamedIndividual rdf:about="http://purl.obolibrary.org/obo/GAZ_00242038">
        <obo:RO_0001025 rdf:resource="http://purl.obolibrary.org/obo/GAZ_00230305"/>
        <obo:IAO_0000115>An administrative region (kism) of 6th of October Governorate.</obo:IAO_0000115>
        <oboInOwl:hasOBONamespace>GAZ</oboInOwl:hasOBONamespace>
        <oboInOwl:id>GAZ:00242038</oboInOwl:id>
        <rdfs:label>Kism Madinat Sittah Uktubar Second</rdfs:label>
    </owl:NamedIndividual>
    


    <!-- http://purl.obolibrary.org/obo/GAZ_00242039 -->

    <owl:NamedIndividual rdf:about="http://purl.obolibrary.org/obo/GAZ_00242039">
        <obo:RO_0001025 rdf:resource="http://purl.obolibrary.org/obo/GAZ_00030916"/>
        <obo:IAO_0000115>An administrative region (markaz) of Damietta Governorate.</obo:IAO_0000115>
        <oboInOwl:hasOBONamespace>GAZ</oboInOwl:hasOBONamespace>
        <oboInOwl:id>GAZ:00242039</oboInOwl:id>
        <rdfs:label>Kism Kafr Sa&apos;d</rdfs:label>
    </owl:NamedIndividual>
    


    <!-- http://purl.obolibrary.org/obo/GAZ_00242040 -->

    <owl:NamedIndividual rdf:about="http://purl.obolibrary.org/obo/GAZ_00242040">
        <obo:RO_0001025 rdf:resource="http://purl.obolibrary.org/obo/GAZ_00030936"/>
        <obo:IAO_0000115>An administrative region (kism) of Sohag Governorate.</obo:IAO_0000115>
        <oboInOwl:hasOBONamespace>GAZ</oboInOwl:hasOBONamespace>
        <oboInOwl:id>GAZ:00242040</oboInOwl:id>
        <rdfs:label>Kism Jirja City</rdfs:label>
    </owl:NamedIndividual>
    


    <!-- http://purl.obolibrary.org/obo/GAZ_00242041 -->

    <owl:NamedIndividual rdf:about="http://purl.obolibrary.org/obo/GAZ_00242041">
        <obo:RO_0001025 rdf:resource="http://purl.obolibrary.org/obo/GAZ_00030933"/>
        <obo:IAO_0000115>An administrative region (kism) of Sohag Governorate.</obo:IAO_0000115>
        <oboInOwl:hasOBONamespace>GAZ</oboInOwl:hasOBONamespace>
        <oboInOwl:id>GAZ:00242041</oboInOwl:id>
        <rdfs:label>Kism Suhaj First</rdfs:label>
    </owl:NamedIndividual>
    


    <!-- http://purl.obolibrary.org/obo/GAZ_00242042 -->

    <owl:NamedIndividual rdf:about="http://purl.obolibrary.org/obo/GAZ_00242042">
        <obo:RO_0001025 rdf:resource="http://purl.obolibrary.org/obo/GAZ_00030933"/>
        <obo:IAO_0000115>An administrative region of Sohag Governorate.</obo:IAO_0000115>
        <oboInOwl:hasOBONamespace>GAZ</oboInOwl:hasOBONamespace>
        <oboInOwl:id>GAZ:00242042</oboInOwl:id>
        <rdfs:label>Suhaj New City</rdfs:label>
    </owl:NamedIndividual>
    


    <!-- http://purl.obolibrary.org/obo/GAZ_00242043 -->

    <owl:NamedIndividual rdf:about="http://purl.obolibrary.org/obo/GAZ_00242043">
        <obo:RO_0001025 rdf:resource="http://purl.obolibrary.org/obo/GAZ_00030933"/>
        <obo:IAO_0000115>An administrative region (kism) of Sohag Governorate.</obo:IAO_0000115>
        <oboInOwl:hasOBONamespace>GAZ</oboInOwl:hasOBONamespace>
        <oboInOwl:id>GAZ:00242043</oboInOwl:id>
        <rdfs:label>Kism Suhaj Second</rdfs:label>
    </owl:NamedIndividual>
    


    <!-- http://purl.obolibrary.org/obo/GAZ_00242044 -->

    <owl:NamedIndividual rdf:about="http://purl.obolibrary.org/obo/GAZ_00242044">
        <obo:RO_0001025 rdf:resource="http://purl.obolibrary.org/obo/GAZ_00030929"/>
        <obo:IAO_0000115>An administrative region (kism) of Sohag Governorate.</obo:IAO_0000115>
        <oboInOwl:hasOBONamespace>GAZ</oboInOwl:hasOBONamespace>
        <oboInOwl:id>GAZ:00242044</oboInOwl:id>
        <rdfs:label>Kism Tahta</rdfs:label>
    </owl:NamedIndividual>
    


    <!-- http://purl.obolibrary.org/obo/GAZ_00242045 -->

    <owl:NamedIndividual rdf:about="http://purl.obolibrary.org/obo/GAZ_00242045">
        <obo:RO_0001025 rdf:resource="http://purl.obolibrary.org/obo/GAZ_00000652"/>
        <obo:IAO_0000115>An administrative region (kism) of Sohag Governorate.</obo:IAO_0000115>
        <oboInOwl:hasOBONamespace>GAZ</oboInOwl:hasOBONamespace>
        <oboInOwl:id>GAZ:00242045</oboInOwl:id>
        <rdfs:label>Kism Al Kawthar</rdfs:label>
    </owl:NamedIndividual>
    


    <!-- http://purl.obolibrary.org/obo/GAZ_00242046 -->

    <owl:NamedIndividual rdf:about="http://purl.obolibrary.org/obo/GAZ_00242046">
        <obo:RO_0001025 rdf:resource="http://purl.obolibrary.org/obo/GAZ_00030957"/>
        <obo:IAO_0000115>An administrative region (kism) of Qena Governorate.</obo:IAO_0000115>
        <oboInOwl:hasOBONamespace>GAZ</oboInOwl:hasOBONamespace>
        <oboInOwl:id>GAZ:00242046</oboInOwl:id>
        <rdfs:label>Kism Qina</rdfs:label>
    </owl:NamedIndividual>
    


    <!-- http://purl.obolibrary.org/obo/GAZ_00242047 -->

    <owl:NamedIndividual rdf:about="http://purl.obolibrary.org/obo/GAZ_00242047">
        <obo:RO_0001025 rdf:resource="http://purl.obolibrary.org/obo/GAZ_00031028"/>
        <obo:IAO_0000115>An administrative region (kism) of Minya Governorate.</obo:IAO_0000115>
        <oboInOwl:hasOBONamespace>GAZ</oboInOwl:hasOBONamespace>
        <oboInOwl:id>GAZ:00242047</oboInOwl:id>
        <rdfs:label>Kism Mallawi</rdfs:label>
    </owl:NamedIndividual>
    


    <!-- http://purl.obolibrary.org/obo/GAZ_00242048 -->

    <owl:NamedIndividual rdf:about="http://purl.obolibrary.org/obo/GAZ_00242048">
        <obo:RO_0001025 rdf:resource="http://purl.obolibrary.org/obo/GAZ_00031027"/>
        <obo:IAO_0000115>An administrative region (kism) of Minya Governorate.</obo:IAO_0000115>
        <oboInOwl:hasOBONamespace>GAZ</oboInOwl:hasOBONamespace>
        <oboInOwl:id>GAZ:00242048</oboInOwl:id>
        <rdfs:label>Kism Al Minya</rdfs:label>
    </owl:NamedIndividual>
    


    <!-- http://purl.obolibrary.org/obo/GAZ_00242049 -->

    <owl:NamedIndividual rdf:about="http://purl.obolibrary.org/obo/GAZ_00242049">
        <obo:RO_0001025 rdf:resource="http://purl.obolibrary.org/obo/GAZ_00031027"/>
        <obo:IAO_0000115>An administrative region of Minya Governorate.</obo:IAO_0000115>
        <oboInOwl:hasOBONamespace>GAZ</oboInOwl:hasOBONamespace>
        <oboInOwl:id>GAZ:00242049</oboInOwl:id>
        <rdfs:label>New Minya City</rdfs:label>
    </owl:NamedIndividual>
    


    <!-- http://purl.obolibrary.org/obo/GAZ_00242050 -->

    <owl:NamedIndividual rdf:about="http://purl.obolibrary.org/obo/GAZ_00242050">
        <obo:RO_0001025 rdf:resource="http://purl.obolibrary.org/obo/GAZ_00000649"/>
        <obo:IAO_0000115>An administrative region (kism) of Giza Governorate.</obo:IAO_0000115>
        <oboInOwl:hasOBONamespace>GAZ</oboInOwl:hasOBONamespace>
        <oboInOwl:id>GAZ:00242050</oboInOwl:id>
        <rdfs:label>Kism Ad Duqqi</rdfs:label>
    </owl:NamedIndividual>
    


    <!-- http://purl.obolibrary.org/obo/GAZ_00242051 -->

    <owl:NamedIndividual rdf:about="http://purl.obolibrary.org/obo/GAZ_00242051">
        <obo:RO_0001025 rdf:resource="http://purl.obolibrary.org/obo/GAZ_00000649"/>
        <obo:IAO_0000115>An administrative region (kism) of Giza Governorate.</obo:IAO_0000115>
        <oboInOwl:hasOBONamespace>GAZ</oboInOwl:hasOBONamespace>
        <oboInOwl:id>GAZ:00242051</oboInOwl:id>
        <rdfs:label>Kism Al &apos;Ajuzah</rdfs:label>
    </owl:NamedIndividual>
    


    <!-- http://purl.obolibrary.org/obo/GAZ_00242052 -->

    <owl:NamedIndividual rdf:about="http://purl.obolibrary.org/obo/GAZ_00242052">
        <obo:RO_0001025 rdf:resource="http://purl.obolibrary.org/obo/GAZ_00000649"/>
        <obo:IAO_0000115>An administrative region (kism) of Giza Governorate.</obo:IAO_0000115>
        <oboInOwl:hasOBONamespace>GAZ</oboInOwl:hasOBONamespace>
        <oboInOwl:id>GAZ:00242052</oboInOwl:id>
        <rdfs:label>Kism Al Harraniyah</rdfs:label>
    </owl:NamedIndividual>
    


    <!-- http://purl.obolibrary.org/obo/GAZ_00242053 -->

    <owl:NamedIndividual rdf:about="http://purl.obolibrary.org/obo/GAZ_00242053">
        <obo:RO_0001025 rdf:resource="http://purl.obolibrary.org/obo/GAZ_00000649"/>
        <obo:IAO_0000115>An administrative region (markaz) of Giza Governorate.</obo:IAO_0000115>
        <oboInOwl:hasOBONamespace>GAZ</oboInOwl:hasOBONamespace>
        <oboInOwl:id>GAZ:00242053</oboInOwl:id>
        <rdfs:label>Al Jizah Region</rdfs:label>
    </owl:NamedIndividual>
    


    <!-- http://purl.obolibrary.org/obo/GAZ_00242054 -->

    <owl:NamedIndividual rdf:about="http://purl.obolibrary.org/obo/GAZ_00242054">
        <obo:RO_0001025 rdf:resource="http://purl.obolibrary.org/obo/GAZ_00242053"/>
        <obo:IAO_0000115>An administrative region (kism) of Giza Governorate.</obo:IAO_0000115>
        <oboInOwl:hasOBONamespace>GAZ</oboInOwl:hasOBONamespace>
        <oboInOwl:id>GAZ:00242054</oboInOwl:id>
        <rdfs:label>Kism Al Jizah</rdfs:label>
    </owl:NamedIndividual>
    


    <!-- http://purl.obolibrary.org/obo/GAZ_00242055 -->

    <owl:NamedIndividual rdf:about="http://purl.obolibrary.org/obo/GAZ_00242055">
        <obo:RO_0001025 rdf:resource="http://purl.obolibrary.org/obo/GAZ_00000649"/>
        <obo:IAO_0000115>An administrative region (kism) of Giza Governorate.</obo:IAO_0000115>
        <oboInOwl:hasOBONamespace>GAZ</oboInOwl:hasOBONamespace>
        <oboInOwl:id>GAZ:00242055</oboInOwl:id>
        <rdfs:label>Kism Al Warraq</rdfs:label>
    </owl:NamedIndividual>
    


    <!-- http://purl.obolibrary.org/obo/GAZ_00242056 -->

    <owl:NamedIndividual rdf:about="http://purl.obolibrary.org/obo/GAZ_00242056">
        <obo:RO_0001025 rdf:resource="http://purl.obolibrary.org/obo/GAZ_00000649"/>
        <obo:IAO_0000115>An administrative region (kism) of Giza Governorate.</obo:IAO_0000115>
        <oboInOwl:hasOBONamespace>GAZ</oboInOwl:hasOBONamespace>
        <oboInOwl:id>GAZ:00242056</oboInOwl:id>
        <rdfs:label>Kism Ash Shaykh Zayid</rdfs:label>
    </owl:NamedIndividual>
    


    <!-- http://purl.obolibrary.org/obo/GAZ_00242057 -->

    <owl:NamedIndividual rdf:about="http://purl.obolibrary.org/obo/GAZ_00242057">
        <obo:RO_0001025 rdf:resource="http://purl.obolibrary.org/obo/GAZ_00000649"/>
        <obo:IAO_0000115>An administrative region (markaz) of Giza Governorate.</obo:IAO_0000115>
        <oboInOwl:hasOBONamespace>GAZ</oboInOwl:hasOBONamespace>
        <oboInOwl:id>GAZ:00242057</oboInOwl:id>
        <rdfs:label>Imbabah Region</rdfs:label>
    </owl:NamedIndividual>
    


    <!-- http://purl.obolibrary.org/obo/GAZ_00242058 -->

    <owl:NamedIndividual rdf:about="http://purl.obolibrary.org/obo/GAZ_00242058">
        <obo:RO_0001025 rdf:resource="http://purl.obolibrary.org/obo/GAZ_00242057"/>
        <obo:IAO_0000115>An administrative region (kism) of Giza Governorate.</obo:IAO_0000115>
        <oboInOwl:hasOBONamespace>GAZ</oboInOwl:hasOBONamespace>
        <oboInOwl:id>GAZ:00242058</oboInOwl:id>
        <rdfs:label>Kism Imbabah</rdfs:label>
    </owl:NamedIndividual>
    


    <!-- http://purl.obolibrary.org/obo/GAZ_00242059 -->

    <owl:NamedIndividual rdf:about="http://purl.obolibrary.org/obo/GAZ_00242059">
        <obo:RO_0001025 rdf:resource="http://purl.obolibrary.org/obo/GAZ_00000649"/>
        <obo:IAO_0000115>An administrative region (markaz) of Giza Governorate.</obo:IAO_0000115>
        <oboInOwl:hasOBONamespace>GAZ</oboInOwl:hasOBONamespace>
        <oboInOwl:id>GAZ:00242059</oboInOwl:id>
        <rdfs:label>Kirdasah Region</rdfs:label>
    </owl:NamedIndividual>
    


    <!-- http://purl.obolibrary.org/obo/GAZ_00242060 -->

    <owl:NamedIndividual rdf:about="http://purl.obolibrary.org/obo/GAZ_00242060">
        <obo:RO_0001025 rdf:resource="http://purl.obolibrary.org/obo/GAZ_00000649"/>
        <obo:IAO_0000115>An administrative region (kism) of Giza Governorate.</obo:IAO_0000115>
        <oboInOwl:hasOBONamespace>GAZ</oboInOwl:hasOBONamespace>
        <oboInOwl:id>GAZ:00242060</oboInOwl:id>
        <rdfs:label>Kism Pyramid</rdfs:label>
    </owl:NamedIndividual>
    


    <!-- http://purl.obolibrary.org/obo/GAZ_00242061 -->

    <owl:NamedIndividual rdf:about="http://purl.obolibrary.org/obo/GAZ_00242061">
        <obo:RO_0001025 rdf:resource="http://purl.obolibrary.org/obo/GAZ_00066384"/>
        <obo:IAO_0000115>An administrative region (kism) of Faiyum Governorate.</obo:IAO_0000115>
        <oboInOwl:hasOBONamespace>GAZ</oboInOwl:hasOBONamespace>
        <oboInOwl:id>GAZ:00242061</oboInOwl:id>
        <rdfs:label>Kism Al Fayyum</rdfs:label>
    </owl:NamedIndividual>
    


    <!-- http://purl.obolibrary.org/obo/GAZ_00242062 -->

    <owl:NamedIndividual rdf:about="http://purl.obolibrary.org/obo/GAZ_00242062">
        <obo:RO_0001025 rdf:resource="http://purl.obolibrary.org/obo/GAZ_00000648"/>
        <obo:IAO_0000115>An administrative region (markaz) of Faiyum Governorate.</obo:IAO_0000115>
        <oboInOwl:hasOBONamespace>GAZ</oboInOwl:hasOBONamespace>
        <oboInOwl:id>GAZ:00242062</oboInOwl:id>
        <rdfs:label>Yusuf Al Sedike Region</rdfs:label>
    </owl:NamedIndividual>
    


    <!-- http://purl.obolibrary.org/obo/GAZ_00242063 -->

    <owl:NamedIndividual rdf:about="http://purl.obolibrary.org/obo/GAZ_00242063">
        <obo:RO_0001025 rdf:resource="http://purl.obolibrary.org/obo/GAZ_00066380"/>
        <obo:IAO_0000115>An administrative region (kism) of Beni Suef Governorate.</obo:IAO_0000115>
        <oboInOwl:hasOBONamespace>GAZ</oboInOwl:hasOBONamespace>
        <oboInOwl:id>GAZ:00242063</oboInOwl:id>
        <rdfs:label>Kism Bani Suwayf</rdfs:label>
    </owl:NamedIndividual>
    


    <!-- http://purl.obolibrary.org/obo/GAZ_00242064 -->

    <owl:NamedIndividual rdf:about="http://purl.obolibrary.org/obo/GAZ_00242064">
        <obo:RO_0001025 rdf:resource="http://purl.obolibrary.org/obo/GAZ_00066380"/>
        <obo:IAO_0000115>An administrative region (kism) of Beni Suef Governorate.</obo:IAO_0000115>
        <oboInOwl:hasOBONamespace>GAZ</oboInOwl:hasOBONamespace>
        <oboInOwl:id>GAZ:00242064</oboInOwl:id>
        <rdfs:label>Kism New Bani Suwayf City</rdfs:label>
    </owl:NamedIndividual>
    


    <!-- http://purl.obolibrary.org/obo/GAZ_00242065 -->

    <owl:NamedIndividual rdf:about="http://purl.obolibrary.org/obo/GAZ_00242065">
        <obo:RO_0001025 rdf:resource="http://purl.obolibrary.org/obo/GAZ_00030996"/>
        <obo:IAO_0000115>An administrative region (kism) of Asyut Governorate.</obo:IAO_0000115>
        <oboInOwl:hasOBONamespace>GAZ</oboInOwl:hasOBONamespace>
        <oboInOwl:id>GAZ:00242065</oboInOwl:id>
        <rdfs:label>Kism Asyut First</rdfs:label>
    </owl:NamedIndividual>
    


    <!-- http://purl.obolibrary.org/obo/GAZ_00242066 -->

    <owl:NamedIndividual rdf:about="http://purl.obolibrary.org/obo/GAZ_00242066">
        <obo:RO_0001025 rdf:resource="http://purl.obolibrary.org/obo/GAZ_00030996"/>
        <obo:IAO_0000115>An administrative region of Asyut Governorate.</obo:IAO_0000115>
        <oboInOwl:hasOBONamespace>GAZ</oboInOwl:hasOBONamespace>
        <oboInOwl:id>GAZ:00242066</oboInOwl:id>
        <rdfs:label>Asyut New City</rdfs:label>
    </owl:NamedIndividual>
    


    <!-- http://purl.obolibrary.org/obo/GAZ_00242067 -->

    <owl:NamedIndividual rdf:about="http://purl.obolibrary.org/obo/GAZ_00242067">
        <obo:RO_0001025 rdf:resource="http://purl.obolibrary.org/obo/GAZ_00030996"/>
        <obo:IAO_0000115>An administrative region (kism) of Asyut Governorate.</obo:IAO_0000115>
        <oboInOwl:hasOBONamespace>GAZ</oboInOwl:hasOBONamespace>
        <oboInOwl:id>GAZ:00242067</oboInOwl:id>
        <rdfs:label>Kism Asyut Second</rdfs:label>
    </owl:NamedIndividual>
    


    <!-- http://purl.obolibrary.org/obo/GAZ_00242068 -->

    <owl:NamedIndividual rdf:about="http://purl.obolibrary.org/obo/GAZ_00242068">
        <obo:RO_0001025 rdf:resource="http://purl.obolibrary.org/obo/GAZ_00066372"/>
        <obo:IAO_0000115>An administrative region (kism) of Aswan Governorate.</obo:IAO_0000115>
        <oboInOwl:hasOBONamespace>GAZ</oboInOwl:hasOBONamespace>
        <oboInOwl:id>GAZ:00242068</oboInOwl:id>
        <rdfs:label>Kism Aswan</rdfs:label>
    </owl:NamedIndividual>
    


    <!-- http://purl.obolibrary.org/obo/GAZ_00242069 -->

    <owl:NamedIndividual rdf:about="http://purl.obolibrary.org/obo/GAZ_00242069">
        <obo:RO_0001025 rdf:resource="http://purl.obolibrary.org/obo/GAZ_00000645"/>
        <obo:IAO_0000115>An administrative region (markaz) of Aswan Governorate.</obo:IAO_0000115>
        <oboInOwl:hasOBONamespace>GAZ</oboInOwl:hasOBONamespace>
        <oboInOwl:id>GAZ:00242069</oboInOwl:id>
        <rdfs:label>Abu Simbel Region</rdfs:label>
    </owl:NamedIndividual>
    


    <!-- http://purl.obolibrary.org/obo/GAZ_00242070 -->

    <owl:NamedIndividual rdf:about="http://purl.obolibrary.org/obo/GAZ_00242070">
        <obo:RO_0001025 rdf:resource="http://purl.obolibrary.org/obo/GAZ_00000645"/>
        <obo:IAO_0000115>An administrative region of Aswan Governorate.</obo:IAO_0000115>
        <oboInOwl:hasOBONamespace>GAZ</oboInOwl:hasOBONamespace>
        <oboInOwl:id>GAZ:00242070</oboInOwl:id>
        <rdfs:label>New Tushka City</rdfs:label>
    </owl:NamedIndividual>
    


    <!-- http://purl.obolibrary.org/obo/GAZ_00242071 -->

    <owl:NamedIndividual rdf:about="http://purl.obolibrary.org/obo/GAZ_00242071">
        <obo:RO_0001025 rdf:resource="http://purl.obolibrary.org/obo/GAZ_00000653"/>
        <obo:IAO_0000115>An administrative region (kism) of Alexandria Governorate.</obo:IAO_0000115>
        <oboInOwl:hasOBONamespace>GAZ</oboInOwl:hasOBONamespace>
        <oboInOwl:id>GAZ:00242071</oboInOwl:id>
        <rdfs:label>Kism New Burj al &apos;Arab</rdfs:label>
    </owl:NamedIndividual>
    


    <!-- http://purl.obolibrary.org/obo/GAZ_00242072 -->

    <owl:NamedIndividual rdf:about="http://purl.obolibrary.org/obo/GAZ_00242072">
        <obo:RO_0001025 rdf:resource="http://purl.obolibrary.org/obo/GAZ_00000653"/>
        <obo:IAO_0000115>An administrative region (kism) of Alexandria Governorate.</obo:IAO_0000115>
        <oboInOwl:hasOBONamespace>GAZ</oboInOwl:hasOBONamespace>
        <oboInOwl:id>GAZ:00242072</oboInOwl:id>
        <rdfs:label>Kism Ad Dukhaylah</rdfs:label>
    </owl:NamedIndividual>
    


    <!-- http://purl.obolibrary.org/obo/GAZ_00242073 -->

    <owl:NamedIndividual rdf:about="http://purl.obolibrary.org/obo/GAZ_00242073">
        <obo:RO_0001025 rdf:resource="http://purl.obolibrary.org/obo/GAZ_00000653"/>
        <obo:IAO_0000115>An administrative region (kism) of Alexandria Governorate.</obo:IAO_0000115>
        <oboInOwl:hasOBONamespace>GAZ</oboInOwl:hasOBONamespace>
        <oboInOwl:id>GAZ:00242073</oboInOwl:id>
        <rdfs:label>Kism Al Manshiyah</rdfs:label>
    </owl:NamedIndividual>
    


    <!-- http://purl.obolibrary.org/obo/GAZ_00242074 -->

    <owl:NamedIndividual rdf:about="http://purl.obolibrary.org/obo/GAZ_00242074">
        <obo:RO_0001025 rdf:resource="http://purl.obolibrary.org/obo/GAZ_00000653"/>
        <obo:IAO_0000115>An administrative region (kism) of Alexandria Governorate.</obo:IAO_0000115>
        <oboInOwl:hasOBONamespace>GAZ</oboInOwl:hasOBONamespace>
        <oboInOwl:id>GAZ:00242074</oboInOwl:id>
        <rdfs:label>Kism Ar Raml</rdfs:label>
    </owl:NamedIndividual>
    


    <!-- http://purl.obolibrary.org/obo/GAZ_00242075 -->

    <owl:NamedIndividual rdf:about="http://purl.obolibrary.org/obo/GAZ_00242075">
        <obo:RO_0001025 rdf:resource="http://purl.obolibrary.org/obo/GAZ_00000653"/>
        <obo:IAO_0000115>An administrative region (kism) of Alexandria Governorate.</obo:IAO_0000115>
        <oboInOwl:hasOBONamespace>GAZ</oboInOwl:hasOBONamespace>
        <oboInOwl:id>GAZ:00242075</oboInOwl:id>
        <rdfs:label>Kism Ar Raml Second</rdfs:label>
    </owl:NamedIndividual>
    


    <!-- http://purl.obolibrary.org/obo/GAZ_00242076 -->

    <owl:NamedIndividual rdf:about="http://purl.obolibrary.org/obo/GAZ_00242076">
        <obo:RO_0001025 rdf:resource="http://purl.obolibrary.org/obo/GAZ_00000653"/>
        <obo:IAO_0000115>An administrative region (kism) of Alexandria Governorate.</obo:IAO_0000115>
        <oboInOwl:hasOBONamespace>GAZ</oboInOwl:hasOBONamespace>
        <oboInOwl:id>GAZ:00242076</oboInOwl:id>
        <rdfs:label>Kism Bab Shark</rdfs:label>
    </owl:NamedIndividual>
    


    <!-- http://purl.obolibrary.org/obo/GAZ_00242077 -->

    <owl:NamedIndividual rdf:about="http://purl.obolibrary.org/obo/GAZ_00242077">
        <obo:RO_0001025 rdf:resource="http://purl.obolibrary.org/obo/GAZ_00000653"/>
        <obo:IAO_0000115>An administrative region (kism) of Alexandria Governorate.</obo:IAO_0000115>
        <oboInOwl:hasOBONamespace>GAZ</oboInOwl:hasOBONamespace>
        <oboInOwl:id>GAZ:00242077</oboInOwl:id>
        <rdfs:label>Kism El Atarin</rdfs:label>
    </owl:NamedIndividual>
    


    <!-- http://purl.obolibrary.org/obo/GAZ_00242078 -->

    <owl:NamedIndividual rdf:about="http://purl.obolibrary.org/obo/GAZ_00242078">
        <obo:RO_0001025 rdf:resource="http://purl.obolibrary.org/obo/GAZ_00000653"/>
        <obo:IAO_0000115>An administrative region (kism) of Alexandria Governorate.</obo:IAO_0000115>
        <oboInOwl:hasOBONamespace>GAZ</oboInOwl:hasOBONamespace>
        <oboInOwl:id>GAZ:00242078</oboInOwl:id>
        <rdfs:label>Kism El Lban</rdfs:label>
    </owl:NamedIndividual>
    


    <!-- http://purl.obolibrary.org/obo/GAZ_00242079 -->

    <owl:NamedIndividual rdf:about="http://purl.obolibrary.org/obo/GAZ_00242079">
        <obo:RO_0001025 rdf:resource="http://purl.obolibrary.org/obo/GAZ_00000653"/>
        <obo:IAO_0000115>An administrative region (kism) of Alexandria Governorate.</obo:IAO_0000115>
        <oboInOwl:hasOBONamespace>GAZ</oboInOwl:hasOBONamespace>
        <oboInOwl:id>GAZ:00242079</oboInOwl:id>
        <rdfs:label>Kism Krowz</rdfs:label>
    </owl:NamedIndividual>
    


    <!-- http://purl.obolibrary.org/obo/GAZ_00242080 -->

    <owl:NamedIndividual rdf:about="http://purl.obolibrary.org/obo/GAZ_00242080">
        <obo:RO_0001025 rdf:resource="http://purl.obolibrary.org/obo/GAZ_00000653"/>
        <obo:IAO_0000115>An administrative region (kism) of Alexandria Governorate.</obo:IAO_0000115>
        <oboInOwl:hasOBONamespace>GAZ</oboInOwl:hasOBONamespace>
        <oboInOwl:id>GAZ:00242080</oboInOwl:id>
        <rdfs:label>Kism Mina&apos; al Basal</rdfs:label>
    </owl:NamedIndividual>
    


    <!-- http://purl.obolibrary.org/obo/GAZ_00242081 -->

    <owl:NamedIndividual rdf:about="http://purl.obolibrary.org/obo/GAZ_00242081">
        <obo:RO_0001025 rdf:resource="http://purl.obolibrary.org/obo/GAZ_00000653"/>
        <obo:IAO_0000115>An administrative region (kism) of Alexandria Governorate.</obo:IAO_0000115>
        <oboInOwl:hasOBONamespace>GAZ</oboInOwl:hasOBONamespace>
        <oboInOwl:id>GAZ:00242081</oboInOwl:id>
        <rdfs:label>Kism Muharram Bey</rdfs:label>
    </owl:NamedIndividual>
    


    <!-- http://purl.obolibrary.org/obo/GAZ_00242082 -->

    <owl:NamedIndividual rdf:about="http://purl.obolibrary.org/obo/GAZ_00242082">
        <obo:RO_0001025 rdf:resource="http://purl.obolibrary.org/obo/GAZ_00000653"/>
        <obo:IAO_0000115>An administrative region of Alexandria Governorate.</obo:IAO_0000115>
        <oboInOwl:hasOBONamespace>GAZ</oboInOwl:hasOBONamespace>
        <oboInOwl:id>GAZ:00242082</oboInOwl:id>
        <rdfs:label>North Coast-Part</rdfs:label>
    </owl:NamedIndividual>
    


    <!-- http://purl.obolibrary.org/obo/GAZ_00242083 -->

    <owl:NamedIndividual rdf:about="http://purl.obolibrary.org/obo/GAZ_00242083">
        <obo:RO_0001025 rdf:resource="http://purl.obolibrary.org/obo/GAZ_00000653"/>
        <obo:IAO_0000115>An administrative region of Alexandria Governorate.</obo:IAO_0000115>
        <oboInOwl:hasOBONamespace>GAZ</oboInOwl:hasOBONamespace>
        <oboInOwl:id>GAZ:00242083</oboInOwl:id>
        <rdfs:label>Port Alexandria Police</rdfs:label>
    </owl:NamedIndividual>
    


    <!-- http://purl.obolibrary.org/obo/GAZ_00242084 -->

    <owl:NamedIndividual rdf:about="http://purl.obolibrary.org/obo/GAZ_00242084">
        <obo:RO_0001025 rdf:resource="http://purl.obolibrary.org/obo/GAZ_00000653"/>
        <obo:IAO_0000115>An administrative region (kism) of Alexandria Governorate.</obo:IAO_0000115>
        <oboInOwl:hasOBONamespace>GAZ</oboInOwl:hasOBONamespace>
        <oboInOwl:id>GAZ:00242084</oboInOwl:id>
        <rdfs:label>Kism Sidi Jabir</rdfs:label>
    </owl:NamedIndividual>
    


    <!-- http://purl.obolibrary.org/obo/GAZ_00242085 -->

    <owl:NamedIndividual rdf:about="http://purl.obolibrary.org/obo/GAZ_00242085">
        <obo:RO_0001025 rdf:resource="http://purl.obolibrary.org/obo/GAZ_00005648"/>
        <obo:IAO_0000115>An administrative region (kism) of Cairo Governorate.</obo:IAO_0000115>
        <oboInOwl:hasOBONamespace>GAZ</oboInOwl:hasOBONamespace>
        <oboInOwl:id>GAZ:00242085</oboInOwl:id>
        <rdfs:label>Kism Madinat an Nasr First</rdfs:label>
    </owl:NamedIndividual>
    


    <!-- http://purl.obolibrary.org/obo/GAZ_00242086 -->

    <owl:NamedIndividual rdf:about="http://purl.obolibrary.org/obo/GAZ_00242086">
        <obo:RO_0001025 rdf:resource="http://purl.obolibrary.org/obo/GAZ_00005648"/>
        <obo:IAO_0000115>An administrative region (kism) of Cairo Governorate.</obo:IAO_0000115>
        <oboInOwl:hasOBONamespace>GAZ</oboInOwl:hasOBONamespace>
        <oboInOwl:id>GAZ:00242086</oboInOwl:id>
        <rdfs:label>Kism Madinat an Nasr Second</rdfs:label>
    </owl:NamedIndividual>
    


    <!-- http://purl.obolibrary.org/obo/GAZ_00242087 -->

    <owl:NamedIndividual rdf:about="http://purl.obolibrary.org/obo/GAZ_00242087">
        <obo:RO_0001025 rdf:resource="http://purl.obolibrary.org/obo/GAZ_00005648"/>
        <obo:IAO_0000115>An administrative region (kism) of Cairo Governorate.</obo:IAO_0000115>
        <oboInOwl:hasOBONamespace>GAZ</oboInOwl:hasOBONamespace>
        <oboInOwl:id>GAZ:00242087</oboInOwl:id>
        <rdfs:label>Kism El Zawia El Hamra</rdfs:label>
    </owl:NamedIndividual>
    


    <!-- http://purl.obolibrary.org/obo/GAZ_00242088 -->

    <owl:NamedIndividual rdf:about="http://purl.obolibrary.org/obo/GAZ_00242088">
        <obo:RO_0001025 rdf:resource="http://purl.obolibrary.org/obo/GAZ_00005648"/>
        <obo:IAO_0000115>An administrative region (kism) of Cairo Governorate.</obo:IAO_0000115>
        <oboInOwl:hasOBONamespace>GAZ</oboInOwl:hasOBONamespace>
        <oboInOwl:id>GAZ:00242088</oboInOwl:id>
        <rdfs:label>Kism El Zawia El Hmra</rdfs:label>
    </owl:NamedIndividual>
    


    <!-- http://purl.obolibrary.org/obo/GAZ_00242089 -->

    <owl:NamedIndividual rdf:about="http://purl.obolibrary.org/obo/GAZ_00242089">
        <obo:RO_0001025 rdf:resource="http://purl.obolibrary.org/obo/GAZ_00005648"/>
        <obo:IAO_0000115>An administrative region (kism) of Cairo Governorate.</obo:IAO_0000115>
        <oboInOwl:hasOBONamespace>GAZ</oboInOwl:hasOBONamespace>
        <oboInOwl:id>GAZ:00242089</oboInOwl:id>
        <rdfs:label>Kism Al Azbakiyah</rdfs:label>
    </owl:NamedIndividual>
    


    <!-- http://purl.obolibrary.org/obo/GAZ_00242090 -->

    <owl:NamedIndividual rdf:about="http://purl.obolibrary.org/obo/GAZ_00242090">
        <obo:RO_0001025 rdf:resource="http://purl.obolibrary.org/obo/GAZ_00005648"/>
        <obo:IAO_0000115>An administrative region (kism) of Cairo Governorate.</obo:IAO_0000115>
        <oboInOwl:hasOBONamespace>GAZ</oboInOwl:hasOBONamespace>
        <oboInOwl:id>GAZ:00242090</oboInOwl:id>
        <rdfs:label>Kism Ancient Cairo</rdfs:label>
    </owl:NamedIndividual>
    


    <!-- http://purl.obolibrary.org/obo/GAZ_00242091 -->

    <owl:NamedIndividual rdf:about="http://purl.obolibrary.org/obo/GAZ_00242091">
        <obo:RO_0001025 rdf:resource="http://purl.obolibrary.org/obo/GAZ_00005648"/>
        <obo:IAO_0000115>An administrative region (kism) of Cairo Governorate.</obo:IAO_0000115>
        <oboInOwl:hasOBONamespace>GAZ</oboInOwl:hasOBONamespace>
        <oboInOwl:id>GAZ:00242091</oboInOwl:id>
        <rdfs:label>Kism Az Zamalik</rdfs:label>
    </owl:NamedIndividual>
    


    <!-- http://purl.obolibrary.org/obo/GAZ_00242092 -->

    <owl:NamedIndividual rdf:about="http://purl.obolibrary.org/obo/GAZ_00242092">
        <obo:RO_0001025 rdf:resource="http://purl.obolibrary.org/obo/GAZ_00005648"/>
        <obo:IAO_0000115>An administrative region (kism) of Cairo Governorate.</obo:IAO_0000115>
        <oboInOwl:hasOBONamespace>GAZ</oboInOwl:hasOBONamespace>
        <oboInOwl:id>GAZ:00242092</oboInOwl:id>
        <rdfs:label>Kism Bulaq</rdfs:label>
    </owl:NamedIndividual>
    


    <!-- http://purl.obolibrary.org/obo/GAZ_00242093 -->

    <owl:NamedIndividual rdf:about="http://purl.obolibrary.org/obo/GAZ_00242093">
        <obo:RO_0001025 rdf:resource="http://purl.obolibrary.org/obo/GAZ_00005648"/>
        <obo:IAO_0000115>An administrative region (kism) of Cairo Governorate.</obo:IAO_0000115>
        <oboInOwl:hasOBONamespace>GAZ</oboInOwl:hasOBONamespace>
        <oboInOwl:id>GAZ:00242093</oboInOwl:id>
        <rdfs:label>Kism El Darb El Ahmr</rdfs:label>
    </owl:NamedIndividual>
    


    <!-- http://purl.obolibrary.org/obo/GAZ_00242094 -->

    <owl:NamedIndividual rdf:about="http://purl.obolibrary.org/obo/GAZ_00242094">
        <obo:RO_0001025 rdf:resource="http://purl.obolibrary.org/obo/GAZ_00005648"/>
        <obo:IAO_0000115>An administrative region (kism) of Cairo Governorate.</obo:IAO_0000115>
        <oboInOwl:hasOBONamespace>GAZ</oboInOwl:hasOBONamespace>
        <oboInOwl:id>GAZ:00242094</oboInOwl:id>
        <rdfs:label>Kism El Khalifa</rdfs:label>
    </owl:NamedIndividual>
    


    <!-- http://purl.obolibrary.org/obo/GAZ_00242095 -->

    <owl:NamedIndividual rdf:about="http://purl.obolibrary.org/obo/GAZ_00242095">
        <obo:RO_0001025 rdf:resource="http://purl.obolibrary.org/obo/GAZ_00005648"/>
        <obo:IAO_0000115>An administrative region (kism) of Cairo Governorate.</obo:IAO_0000115>
        <oboInOwl:hasOBONamespace>GAZ</oboInOwl:hasOBONamespace>
        <oboInOwl:id>GAZ:00242095</oboInOwl:id>
        <rdfs:label>Kism El Mosky</rdfs:label>
    </owl:NamedIndividual>
    


    <!-- http://purl.obolibrary.org/obo/GAZ_00242096 -->

    <owl:NamedIndividual rdf:about="http://purl.obolibrary.org/obo/GAZ_00242096">
        <obo:RO_0001025 rdf:resource="http://purl.obolibrary.org/obo/GAZ_00005648"/>
        <obo:IAO_0000115>An administrative region (kism) of Cairo Governorate.</obo:IAO_0000115>
        <oboInOwl:hasOBONamespace>GAZ</oboInOwl:hasOBONamespace>
        <oboInOwl:id>GAZ:00242096</oboInOwl:id>
        <rdfs:label>Kism El Nozha</rdfs:label>
    </owl:NamedIndividual>
    


    <!-- http://purl.obolibrary.org/obo/GAZ_00242097 -->

    <owl:NamedIndividual rdf:about="http://purl.obolibrary.org/obo/GAZ_00242097">
        <obo:RO_0001025 rdf:resource="http://purl.obolibrary.org/obo/GAZ_00005648"/>
        <obo:IAO_0000115>An administrative region (kism) of Cairo Governorate.</obo:IAO_0000115>
        <oboInOwl:hasOBONamespace>GAZ</oboInOwl:hasOBONamespace>
        <oboInOwl:id>GAZ:00242097</oboInOwl:id>
        <rdfs:label>Kism El Tbin</rdfs:label>
    </owl:NamedIndividual>
    


    <!-- http://purl.obolibrary.org/obo/GAZ_00242098 -->

    <owl:NamedIndividual rdf:about="http://purl.obolibrary.org/obo/GAZ_00242098">
        <obo:RO_0001025 rdf:resource="http://purl.obolibrary.org/obo/GAZ_00005648"/>
        <obo:IAO_0000115>An administrative region (kism) of Cairo Governorate.</obo:IAO_0000115>
        <oboInOwl:hasOBONamespace>GAZ</oboInOwl:hasOBONamespace>
        <oboInOwl:id>GAZ:00242098</oboInOwl:id>
        <rdfs:label>Kism El Zahe</rdfs:label>
    </owl:NamedIndividual>
    


    <!-- http://purl.obolibrary.org/obo/GAZ_00242099 -->

    <owl:NamedIndividual rdf:about="http://purl.obolibrary.org/obo/GAZ_00242099">
        <obo:RO_0001025 rdf:resource="http://purl.obolibrary.org/obo/GAZ_00005648"/>
        <obo:IAO_0000115>An administrative region (kism) of Cairo Governorate.</obo:IAO_0000115>
        <oboInOwl:hasOBONamespace>GAZ</oboInOwl:hasOBONamespace>
        <oboInOwl:id>GAZ:00242099</oboInOwl:id>
        <rdfs:label>Kism Elgamalia</rdfs:label>
    </owl:NamedIndividual>
    


    <!-- http://purl.obolibrary.org/obo/GAZ_00242100 -->

    <owl:NamedIndividual rdf:about="http://purl.obolibrary.org/obo/GAZ_00242100">
        <obo:RO_0001025 rdf:resource="http://purl.obolibrary.org/obo/GAZ_00005648"/>
        <obo:IAO_0000115>An administrative region (kism) of Cairo Governorate.</obo:IAO_0000115>
        <oboInOwl:hasOBONamespace>GAZ</oboInOwl:hasOBONamespace>
        <oboInOwl:id>GAZ:00242100</oboInOwl:id>
        <rdfs:label>Kism Heliopolis</rdfs:label>
    </owl:NamedIndividual>
    


    <!-- http://purl.obolibrary.org/obo/GAZ_00242101 -->

    <owl:NamedIndividual rdf:about="http://purl.obolibrary.org/obo/GAZ_00242101">
        <obo:RO_0001025 rdf:resource="http://purl.obolibrary.org/obo/GAZ_00005648"/>
        <obo:IAO_0000115>An administrative region (kism) of Cairo Governorate.</obo:IAO_0000115>
        <oboInOwl:hasOBONamespace>GAZ</oboInOwl:hasOBONamespace>
        <oboInOwl:id>GAZ:00242101</oboInOwl:id>
        <rdfs:label>Kism Kasr El Nile</rdfs:label>
    </owl:NamedIndividual>
    


    <!-- http://purl.obolibrary.org/obo/GAZ_00242102 -->

    <owl:NamedIndividual rdf:about="http://purl.obolibrary.org/obo/GAZ_00242102">
        <obo:RO_0001025 rdf:resource="http://purl.obolibrary.org/obo/GAZ_00005648"/>
        <obo:IAO_0000115>An administrative region (kism) of Cairo Governorate.</obo:IAO_0000115>
        <oboInOwl:hasOBONamespace>GAZ</oboInOwl:hasOBONamespace>
        <oboInOwl:id>GAZ:00242102</oboInOwl:id>
        <rdfs:label>Kism Tura</rdfs:label>
    </owl:NamedIndividual>
    


    <!-- http://purl.obolibrary.org/obo/GAZ_00242103 -->

    <owl:NamedIndividual rdf:about="http://purl.obolibrary.org/obo/GAZ_00242103">
        <obo:RO_0001025 rdf:resource="http://purl.obolibrary.org/obo/GAZ_00230304"/>
        <obo:IAO_0000115>An administrative region (kism) of Helwan Governorate.</obo:IAO_0000115>
        <oboInOwl:hasOBONamespace>GAZ</oboInOwl:hasOBONamespace>
        <oboInOwl:id>GAZ:00242103</oboInOwl:id>
        <rdfs:label>Kism Al Ma&apos;adi</rdfs:label>
    </owl:NamedIndividual>
    


    <!-- http://purl.obolibrary.org/obo/GAZ_00242104 -->

    <owl:NamedIndividual rdf:about="http://purl.obolibrary.org/obo/GAZ_00242104">
        <obo:RO_0001025 rdf:resource="http://purl.obolibrary.org/obo/GAZ_00230304"/>
        <obo:IAO_0000115>An administrative region (kism) of Helwan Governorate.</obo:IAO_0000115>
        <oboInOwl:hasOBONamespace>GAZ</oboInOwl:hasOBONamespace>
        <oboInOwl:id>GAZ:00242104</oboInOwl:id>
        <rdfs:label>Kism New Cairo First</rdfs:label>
    </owl:NamedIndividual>
    


    <!-- http://purl.obolibrary.org/obo/GAZ_00242105 -->

    <owl:NamedIndividual rdf:about="http://purl.obolibrary.org/obo/GAZ_00242105">
        <obo:RO_0001025 rdf:resource="http://purl.obolibrary.org/obo/GAZ_00230304"/>
        <obo:IAO_0000115>An administrative region (kism) of Helwan Governorate.</obo:IAO_0000115>
        <oboInOwl:hasOBONamespace>GAZ</oboInOwl:hasOBONamespace>
        <oboInOwl:id>GAZ:00242105</oboInOwl:id>
        <rdfs:label>Kism New Cairo Second</rdfs:label>
    </owl:NamedIndividual>
    


    <!-- http://purl.obolibrary.org/obo/GAZ_00242106 -->

    <owl:NamedIndividual rdf:about="http://purl.obolibrary.org/obo/GAZ_00242106">
        <obo:RO_0001025 rdf:resource="http://purl.obolibrary.org/obo/GAZ_00230304"/>
        <obo:IAO_0000115>An administrative region (kism) of Helwan Governorate.</obo:IAO_0000115>
        <oboInOwl:hasOBONamespace>GAZ</oboInOwl:hasOBONamespace>
        <oboInOwl:id>GAZ:00242106</oboInOwl:id>
        <rdfs:label>Kism New Cairo Third</rdfs:label>
    </owl:NamedIndividual>
    


    <!-- http://purl.obolibrary.org/obo/GAZ_00242107 -->

    <owl:NamedIndividual rdf:about="http://purl.obolibrary.org/obo/GAZ_00242107">
        <obo:RO_0001025 rdf:resource="http://purl.obolibrary.org/obo/GAZ_00230304"/>
        <obo:IAO_0000115>An administrative region (kism) of Helwan Governorate.</obo:IAO_0000115>
        <oboInOwl:hasOBONamespace>GAZ</oboInOwl:hasOBONamespace>
        <oboInOwl:id>GAZ:00242107</oboInOwl:id>
        <rdfs:label>Kism Badr</rdfs:label>
    </owl:NamedIndividual>
    


    <!-- http://purl.obolibrary.org/obo/GAZ_00242108 -->

    <owl:NamedIndividual rdf:about="http://purl.obolibrary.org/obo/GAZ_00242108">
        <obo:RO_0001025 rdf:resource="http://purl.obolibrary.org/obo/GAZ_00230304"/>
        <obo:IAO_0000115>An administrative region (kism) of Helwan Governorate.</obo:IAO_0000115>
        <oboInOwl:hasOBONamespace>GAZ</oboInOwl:hasOBONamespace>
        <oboInOwl:id>GAZ:00242108</oboInOwl:id>
        <rdfs:label>Kism Al Shorouk</rdfs:label>
    </owl:NamedIndividual>
    


    <!-- http://purl.obolibrary.org/obo/GAZ_00242109 -->

    <owl:NamedIndividual rdf:about="http://purl.obolibrary.org/obo/GAZ_00242109">
        <obo:RO_0001025 rdf:resource="http://purl.obolibrary.org/obo/GAZ_00230304"/>
        <obo:IAO_0000115>An administrative region (kism) of Helwan Governorate.</obo:IAO_0000115>
        <oboInOwl:hasOBONamespace>GAZ</oboInOwl:hasOBONamespace>
        <oboInOwl:id>GAZ:00242109</oboInOwl:id>
        <rdfs:label>Kism Badr Section</rdfs:label>
    </owl:NamedIndividual>
    


    <!-- http://purl.obolibrary.org/obo/GAZ_00242110 -->

    <owl:NamedIndividual rdf:about="http://purl.obolibrary.org/obo/GAZ_00242110">
        <obo:RO_0001025 rdf:resource="http://purl.obolibrary.org/obo/GAZ_00230304"/>
        <obo:IAO_0000115>An administrative region of Helwan Governorate.</obo:IAO_0000115>
        <oboInOwl:hasOBONamespace>GAZ</oboInOwl:hasOBONamespace>
        <oboInOwl:id>GAZ:00242110</oboInOwl:id>
        <rdfs:label>Haikstep</rdfs:label>
    </owl:NamedIndividual>
    


    <!-- http://purl.obolibrary.org/obo/GAZ_00242111 -->

    <owl:NamedIndividual rdf:about="http://purl.obolibrary.org/obo/GAZ_00242111">
        <obo:RO_0001025 rdf:resource="http://purl.obolibrary.org/obo/GAZ_00066402"/>
        <obo:IAO_0000115>An administrative region (kism) of Luxor Governorate.</obo:IAO_0000115>
        <oboInOwl:hasOBONamespace>GAZ</oboInOwl:hasOBONamespace>
        <oboInOwl:id>GAZ:00242111</oboInOwl:id>
        <rdfs:label>Kism Al Uqsur</rdfs:label>
    </owl:NamedIndividual>
    


    <!-- http://purl.obolibrary.org/obo/GAZ_00242112 -->

    <owl:NamedIndividual rdf:about="http://purl.obolibrary.org/obo/GAZ_00242112">
        <obo:RO_0001025 rdf:resource="http://purl.obolibrary.org/obo/GAZ_00066400"/>
        <obo:IAO_0000115>An administrative region (markaz) of Luxor Governorate.</obo:IAO_0000115>
        <oboInOwl:hasOBONamespace>GAZ</oboInOwl:hasOBONamespace>
        <oboInOwl:id>GAZ:00242112</oboInOwl:id>
        <rdfs:label>Tiba Shorta Region</rdfs:label>
    </owl:NamedIndividual>
    


    <!-- http://purl.obolibrary.org/obo/GAZ_00242113 -->

    <owl:NamedIndividual rdf:about="http://purl.obolibrary.org/obo/GAZ_00242113">
        <obo:RO_0001025 rdf:resource="http://purl.obolibrary.org/obo/GAZ_00030981"/>
        <obo:IAO_0000115>An administrative region (kism) of Port Said Governorate.</obo:IAO_0000115>
        <oboInOwl:hasOBONamespace>GAZ</oboInOwl:hasOBONamespace>
        <oboInOwl:id>GAZ:00242113</oboInOwl:id>
        <rdfs:label>Kism Mubarak East</rdfs:label>
    </owl:NamedIndividual>
    


    <!-- http://purl.obolibrary.org/obo/GAZ_00242114 -->

    <owl:NamedIndividual rdf:about="http://purl.obolibrary.org/obo/GAZ_00242114">
        <obo:RO_0001025 rdf:resource="http://purl.obolibrary.org/obo/GAZ_00030981"/>
        <obo:IAO_0000115>An administrative region (kism) of Port Said Governorate.</obo:IAO_0000115>
        <oboInOwl:hasOBONamespace>GAZ</oboInOwl:hasOBONamespace>
        <oboInOwl:id>GAZ:00242114</oboInOwl:id>
        <rdfs:label>Kism El Shark</rdfs:label>
    </owl:NamedIndividual>
    


    <!-- http://purl.obolibrary.org/obo/GAZ_00242115 -->

    <owl:NamedIndividual rdf:about="http://purl.obolibrary.org/obo/GAZ_00242115">
        <obo:RO_0001025 rdf:resource="http://purl.obolibrary.org/obo/GAZ_00030981"/>
        <obo:IAO_0000115>An administrative region (kism) of Port Said Governorate.</obo:IAO_0000115>
        <oboInOwl:hasOBONamespace>GAZ</oboInOwl:hasOBONamespace>
        <oboInOwl:id>GAZ:00242115</oboInOwl:id>
        <rdfs:label>Kism Mansra</rdfs:label>
    </owl:NamedIndividual>
    


    <!-- http://purl.obolibrary.org/obo/GAZ_00242116 -->

    <owl:NamedIndividual rdf:about="http://purl.obolibrary.org/obo/GAZ_00242116">
        <obo:RO_0001025 rdf:resource="http://purl.obolibrary.org/obo/GAZ_00030981"/>
        <obo:IAO_0000115>An administrative region (kism) of Port Said Governorate.</obo:IAO_0000115>
        <oboInOwl:hasOBONamespace>GAZ</oboInOwl:hasOBONamespace>
        <oboInOwl:id>GAZ:00242116</oboInOwl:id>
        <rdfs:label>Kism Bur Fu&apos;ad Second</rdfs:label>
    </owl:NamedIndividual>
    


    <!-- http://purl.obolibrary.org/obo/GAZ_00242117 -->

    <owl:NamedIndividual rdf:about="http://purl.obolibrary.org/obo/GAZ_00242117">
        <obo:RO_0001025 rdf:resource="http://purl.obolibrary.org/obo/GAZ_00030981"/>
        <obo:IAO_0000115>An administrative region (kism) of Port Said Governorate.</obo:IAO_0000115>
        <oboInOwl:hasOBONamespace>GAZ</oboInOwl:hasOBONamespace>
        <oboInOwl:id>GAZ:00242117</oboInOwl:id>
        <rdfs:label>Kism Bur Sa&apos;id Police Department</rdfs:label>
    </owl:NamedIndividual>
    


    <!-- http://purl.obolibrary.org/obo/GAZ_00242118 -->

    <owl:NamedIndividual rdf:about="http://purl.obolibrary.org/obo/GAZ_00242118">
        <obo:RO_0001025 rdf:resource="http://purl.obolibrary.org/obo/GAZ_00030981"/>
        <obo:IAO_0000115>An administrative region (kism) of Port Said Governorate.</obo:IAO_0000115>
        <oboInOwl:hasOBONamespace>GAZ</oboInOwl:hasOBONamespace>
        <oboInOwl:id>GAZ:00242118</oboInOwl:id>
        <rdfs:label>Kism Janub Second</rdfs:label>
    </owl:NamedIndividual>
    


    <!-- http://purl.obolibrary.org/obo/GAZ_00242119 -->

    <owl:NamedIndividual rdf:about="http://purl.obolibrary.org/obo/GAZ_00242119">
        <obo:RO_0001025 rdf:resource="http://purl.obolibrary.org/obo/GAZ_00000666"/>
        <obo:IAO_0000115>An administrative region (kism) of Suez Governorate.</obo:IAO_0000115>
        <oboInOwl:hasOBONamespace>GAZ</oboInOwl:hasOBONamespace>
        <oboInOwl:id>GAZ:00242119</oboInOwl:id>
        <rdfs:label>Kism El 40</rdfs:label>
    </owl:NamedIndividual>
    


    <!-- http://purl.obolibrary.org/obo/GAZ_00242120 -->

    <owl:NamedIndividual rdf:about="http://purl.obolibrary.org/obo/GAZ_00242120">
        <obo:RO_0001025 rdf:resource="http://purl.obolibrary.org/obo/GAZ_00000666"/>
        <obo:IAO_0000115>An administrative region (kism) of Suez Governorate.</obo:IAO_0000115>
        <oboInOwl:hasOBONamespace>GAZ</oboInOwl:hasOBONamespace>
        <oboInOwl:id>GAZ:00242120</oboInOwl:id>
        <rdfs:label>Kism Faisal</rdfs:label>
    </owl:NamedIndividual>
    


    <!-- http://purl.obolibrary.org/obo/GAZ_00246604 -->

    <owl:NamedIndividual rdf:about="http://purl.obolibrary.org/obo/GAZ_00246604">
        <obo:IAO_0000115>A freshwater lake. One of the most isolated occurrences of free surface water in the Sahara. It is situated near the southwestern extremity of the plateau, Adrar Nahalet, which extends westwards from the massif of the A&apos;Haggar. The permanent guelta (pool), 13 m wide when full and 6 m deep, is inside a volcanic crater which partly encloses a valley. It collects water from two oueds which drain Ziza Mountain, to the south, and is reputed to have no underground input. Several small temporary pools also occur in the bed of the main oued draining Mount Ziza.</obo:IAO_0000115>
        <oboInOwl:hasOBONamespace>GAZ</oboInOwl:hasOBONamespace>
        <oboInOwl:id>GAZ:00246604</oboInOwl:id>
        <rdfs:label>Gueltas of Ziza</rdfs:label>
    </owl:NamedIndividual>
    


    <!-- http://purl.obolibrary.org/obo/GAZ_00247178 -->

    <owl:NamedIndividual rdf:about="http://purl.obolibrary.org/obo/GAZ_00247178">
        <obo:IAO_0000115>A depression.</obo:IAO_0000115>
        <oboInOwl:hasOBONamespace>GAZ</oboInOwl:hasOBONamespace>
        <oboInOwl:id>GAZ:00247178</oboInOwl:id>
        <rdfs:label>Depression du Mourdi</rdfs:label>
    </owl:NamedIndividual>
    


    <!-- http://purl.obolibrary.org/obo/GAZ_00247180 -->

    <owl:NamedIndividual rdf:about="http://purl.obolibrary.org/obo/GAZ_00247180">
        <obo:IAO_0000115>A mountain range.</obo:IAO_0000115>
        <oboInOwl:hasOBONamespace>GAZ</oboInOwl:hasOBONamespace>
        <oboInOwl:id>GAZ:00247180</oboInOwl:id>
        <rdfs:label>Massif du Kerkour Nourene</rdfs:label>
    </owl:NamedIndividual>
    


    <!-- http://purl.obolibrary.org/obo/GAZ_00247676 -->

    <owl:NamedIndividual rdf:about="http://purl.obolibrary.org/obo/GAZ_00247676">
        <obo:IAO_0000115>An intermittent river in the Sahara.</obo:IAO_0000115>
        <oboInOwl:hasOBONamespace>GAZ</oboInOwl:hasOBONamespace>
        <oboInOwl:id>GAZ:00247676</oboInOwl:id>
        <rdfs:label>Oued Saoura</rdfs:label>
    </owl:NamedIndividual>
    


    <!-- http://purl.obolibrary.org/obo/GAZ_00247997 -->

    <owl:NamedIndividual rdf:about="http://purl.obolibrary.org/obo/GAZ_00247997">
        <obo:RO_0001025 rdf:resource="http://purl.obolibrary.org/obo/GAZ_00000649"/>
        <obo:RO_0001025 rdf:resource="http://purl.obolibrary.org/obo/GAZ_00009949"/>
        <obo:IAO_0000115>A lake.</obo:IAO_0000115>
        <oboInOwl:hasOBONamespace>GAZ</oboInOwl:hasOBONamespace>
        <oboInOwl:id>GAZ:00247997</oboInOwl:id>
        <rdfs:label>Birkat al Mallah</rdfs:label>
    </owl:NamedIndividual>
    


    <!-- http://purl.obolibrary.org/obo/GAZ_00247998 -->

    <owl:NamedIndividual rdf:about="http://purl.obolibrary.org/obo/GAZ_00247998">
        <obo:RO_0001025 rdf:resource="http://purl.obolibrary.org/obo/GAZ_00000649"/>
        <obo:RO_0001025 rdf:resource="http://purl.obolibrary.org/obo/GAZ_00009949"/>
        <obo:IAO_0000115>A lake.</obo:IAO_0000115>
        <oboInOwl:hasOBONamespace>GAZ</oboInOwl:hasOBONamespace>
        <oboInOwl:id>GAZ:00247998</oboInOwl:id>
        <rdfs:label>Birkat al Qatta</rdfs:label>
    </owl:NamedIndividual>
    


    <!-- http://purl.obolibrary.org/obo/GAZ_00247999 -->

    <owl:NamedIndividual rdf:about="http://purl.obolibrary.org/obo/GAZ_00247999">
        <obo:RO_0001025 rdf:resource="http://purl.obolibrary.org/obo/GAZ_00009949"/>
        <obo:IAO_0000115>A lake.</obo:IAO_0000115>
        <oboInOwl:hasOBONamespace>GAZ</oboInOwl:hasOBONamespace>
        <oboInOwl:id>GAZ:00247999</oboInOwl:id>
        <rdfs:label>Lake Faraontya</rdfs:label>
    </owl:NamedIndividual>
    


    <!-- http://purl.obolibrary.org/obo/GAZ_00248000 -->

    <owl:NamedIndividual rdf:about="http://purl.obolibrary.org/obo/GAZ_00248000">
        <obo:RO_0001025 rdf:resource="http://purl.obolibrary.org/obo/GAZ_00009949"/>
        <obo:RO_0001025 rdf:resource="http://purl.obolibrary.org/obo/GAZ_00066411"/>
        <obo:IAO_0000115>A coastal lagoon.</obo:IAO_0000115>
        <oboInOwl:hasOBONamespace>GAZ</oboInOwl:hasOBONamespace>
        <oboInOwl:id>GAZ:00248000</oboInOwl:id>
        <rdfs:label>Buhayrat al Manzilah</rdfs:label>
    </owl:NamedIndividual>
    


    <!-- http://purl.obolibrary.org/obo/GAZ_00248001 -->

    <owl:NamedIndividual rdf:about="http://purl.obolibrary.org/obo/GAZ_00248001">
        <obo:RO_0001025 rdf:resource="http://purl.obolibrary.org/obo/GAZ_00009949"/>
        <obo:IAO_0000115>A lake.</obo:IAO_0000115>
        <oboInOwl:hasOBONamespace>GAZ</oboInOwl:hasOBONamespace>
        <oboInOwl:id>GAZ:00248001</oboInOwl:id>
        <rdfs:label>Birkat Muhayshir</rdfs:label>
    </owl:NamedIndividual>
    


    <!-- http://purl.obolibrary.org/obo/GAZ_00248002 -->

    <owl:NamedIndividual rdf:about="http://purl.obolibrary.org/obo/GAZ_00248002">
        <obo:RO_0001025 rdf:resource="http://purl.obolibrary.org/obo/GAZ_00000655"/>
        <obo:IAO_0000115>A shallow brackish lake. Located 15 km SW of the mouth of the Rosetta branch of the Nile.</obo:IAO_0000115>
        <oboInOwl:hasOBONamespace>GAZ</oboInOwl:hasOBONamespace>
        <oboInOwl:id>GAZ:00248002</oboInOwl:id>
        <rdfs:label>Buhayrat Idku</rdfs:label>
    </owl:NamedIndividual>
    


    <!-- http://purl.obolibrary.org/obo/GAZ_00248004 -->

    <owl:NamedIndividual rdf:about="http://purl.obolibrary.org/obo/GAZ_00248004">
        <obo:RO_0001025 rdf:resource="http://purl.obolibrary.org/obo/GAZ_00000669"/>
        <obo:IAO_0000115>A salt water lagoon, 90 km long and up to 24 km wide, on the Mediterranean coast of Sinai.</obo:IAO_0000115>
        <oboInOwl:hasOBONamespace>GAZ</oboInOwl:hasOBONamespace>
        <oboInOwl:id>GAZ:00248004</oboInOwl:id>
        <rdfs:label>Sabkhet el Bardawil</rdfs:label>
    </owl:NamedIndividual>
    


    <!-- http://purl.obolibrary.org/obo/GAZ_00248005 -->

    <owl:NamedIndividual rdf:about="http://purl.obolibrary.org/obo/GAZ_00248005">
        <obo:RO_0001025 rdf:resource="http://purl.obolibrary.org/obo/GAZ_00002456"/>
        <obo:RO_0001025 rdf:resource="http://purl.obolibrary.org/obo/GAZ_00066415"/>
        <obo:IAO_0000115>An island offshore Al Ghardaqah.</obo:IAO_0000115>
        <oboInOwl:hasOBONamespace>GAZ</oboInOwl:hasOBONamespace>
        <oboInOwl:id>GAZ:00248005</oboInOwl:id>
        <rdfs:label>Abu Minciar Island</rdfs:label>
    </owl:NamedIndividual>
    


    <!-- http://purl.obolibrary.org/obo/GAZ_00248006 -->

    <owl:NamedIndividual rdf:about="http://purl.obolibrary.org/obo/GAZ_00248006">
        <obo:RO_0001025 rdf:resource="http://purl.obolibrary.org/obo/GAZ_00002456"/>
        <obo:RO_0001025 rdf:resource="http://purl.obolibrary.org/obo/GAZ_00066413"/>
        <obo:IAO_0000115>An island offshore Port Sataga.</obo:IAO_0000115>
        <oboInOwl:hasOBONamespace>GAZ</oboInOwl:hasOBONamespace>
        <oboInOwl:id>GAZ:00248006</oboInOwl:id>
        <rdfs:label>Safaga Island</rdfs:label>
    </owl:NamedIndividual>
    


    <!-- http://purl.obolibrary.org/obo/GAZ_00248007 -->

    <owl:NamedIndividual rdf:about="http://purl.obolibrary.org/obo/GAZ_00248007">
        <obo:RO_0001025 rdf:resource="http://purl.obolibrary.org/obo/GAZ_00000654"/>
        <obo:RO_0001025 rdf:resource="http://purl.obolibrary.org/obo/GAZ_00002456"/>
        <obo:IAO_0000115>An island.</obo:IAO_0000115>
        <oboInOwl:hasOBONamespace>GAZ</oboInOwl:hasOBONamespace>
        <oboInOwl:id>GAZ:00248007</oboInOwl:id>
        <rdfs:label>Jazirat Wadi Jimal</rdfs:label>
    </owl:NamedIndividual>
    


    <!-- http://purl.obolibrary.org/obo/GAZ_00248008 -->

    <owl:NamedIndividual rdf:about="http://purl.obolibrary.org/obo/GAZ_00248008">
        <obo:RO_0001025 rdf:resource="http://purl.obolibrary.org/obo/GAZ_00000654"/>
        <obo:IAO_0000115>A river that drains the northern end of the Gebel Hamada Range (1977 masl) and reaches the sea in a bay, the mouth of which is sheltered by Wadi Gimal Island.</obo:IAO_0000115>
        <oboInOwl:hasOBONamespace>GAZ</oboInOwl:hasOBONamespace>
        <oboInOwl:id>GAZ:00248008</oboInOwl:id>
        <rdfs:label>Wadi Gimal</rdfs:label>
    </owl:NamedIndividual>
    


    <!-- http://purl.obolibrary.org/obo/GAZ_00248009 -->

    <owl:NamedIndividual rdf:about="http://purl.obolibrary.org/obo/GAZ_00248009">
        <obo:RO_0001025 rdf:resource="http://purl.obolibrary.org/obo/GAZ_00000667"/>
        <obo:RO_0001025 rdf:resource="http://purl.obolibrary.org/obo/GAZ_00051197"/>
        <obo:IAO_0000115>A depression, about 25 m below sea level at its deepest. Bounded by steep slopes on the northern side, reaching about 120-160 m asl, but by much gentler slopes to the south and southeast.</obo:IAO_0000115>
        <oboInOwl:hasOBONamespace>GAZ</oboInOwl:hasOBONamespace>
        <oboInOwl:id>GAZ:00248009</oboInOwl:id>
        <rdfs:label>Siwa Depression</rdfs:label>
    </owl:NamedIndividual>
    


    <!-- http://purl.obolibrary.org/obo/GAZ_00248010 -->

    <owl:NamedIndividual rdf:about="http://purl.obolibrary.org/obo/GAZ_00248010">
        <obo:RO_0001025 rdf:resource="http://purl.obolibrary.org/obo/GAZ_00248009"/>
        <obo:IAO_0000115>An oasis.</obo:IAO_0000115>
        <oboInOwl:hasOBONamespace>GAZ</oboInOwl:hasOBONamespace>
        <oboInOwl:id>GAZ:00248010</oboInOwl:id>
        <rdfs:label>Shiyata</rdfs:label>
    </owl:NamedIndividual>
    


    <!-- http://purl.obolibrary.org/obo/GAZ_00248011 -->

    <owl:NamedIndividual rdf:about="http://purl.obolibrary.org/obo/GAZ_00248011">
        <obo:RO_0001025 rdf:resource="http://purl.obolibrary.org/obo/GAZ_00248009"/>
        <obo:IAO_0000115>A saline lake.</obo:IAO_0000115>
        <oboInOwl:hasOBONamespace>GAZ</oboInOwl:hasOBONamespace>
        <oboInOwl:id>GAZ:00248011</oboInOwl:id>
        <rdfs:label>Birkat al Maraqi</rdfs:label>
    </owl:NamedIndividual>
    


    <!-- http://purl.obolibrary.org/obo/GAZ_00248012 -->

    <owl:NamedIndividual rdf:about="http://purl.obolibrary.org/obo/GAZ_00248012">
        <obo:RO_0001025 rdf:resource="http://purl.obolibrary.org/obo/GAZ_00248009"/>
        <obo:IAO_0000115>A saline lake.</obo:IAO_0000115>
        <oboInOwl:hasOBONamespace>GAZ</oboInOwl:hasOBONamespace>
        <oboInOwl:id>GAZ:00248012</oboInOwl:id>
        <rdfs:label>Birkat el Zaytun</rdfs:label>
    </owl:NamedIndividual>
    


    <!-- http://purl.obolibrary.org/obo/GAZ_00248013 -->

    <owl:NamedIndividual rdf:about="http://purl.obolibrary.org/obo/GAZ_00248013">
        <obo:RO_0001025 rdf:resource="http://purl.obolibrary.org/obo/GAZ_00248009"/>
        <obo:IAO_0000115>A saline lake.</obo:IAO_0000115>
        <oboInOwl:hasOBONamespace>GAZ</oboInOwl:hasOBONamespace>
        <oboInOwl:id>GAZ:00248013</oboInOwl:id>
        <rdfs:label>Birkat Siwah</rdfs:label>
    </owl:NamedIndividual>
    


    <!-- http://purl.obolibrary.org/obo/GAZ_00248014 -->

    <owl:NamedIndividual rdf:about="http://purl.obolibrary.org/obo/GAZ_00248014">
        <obo:RO_0001025 rdf:resource="http://purl.obolibrary.org/obo/GAZ_00248009"/>
        <obo:IAO_0000115>A saline lake.</obo:IAO_0000115>
        <oboInOwl:hasOBONamespace>GAZ</oboInOwl:hasOBONamespace>
        <oboInOwl:id>GAZ:00248014</oboInOwl:id>
        <rdfs:label>Birkat Aghurmi</rdfs:label>
    </owl:NamedIndividual>
    


    <!-- http://purl.obolibrary.org/obo/GAZ_00248015 -->

    <owl:NamedIndividual rdf:about="http://purl.obolibrary.org/obo/GAZ_00248015">
        <obo:RO_0001025 rdf:resource="http://purl.obolibrary.org/obo/GAZ_00248009"/>
        <obo:IAO_0000115>A saline lake.</obo:IAO_0000115>
        <oboInOwl:hasOBONamespace>GAZ</oboInOwl:hasOBONamespace>
        <oboInOwl:id>GAZ:00248015</oboInOwl:id>
        <rdfs:label>Birkat Samar Abu Ishaq</rdfs:label>
    </owl:NamedIndividual>
    


    <!-- http://purl.obolibrary.org/obo/GAZ_00248016 -->

    <owl:NamedIndividual rdf:about="http://purl.obolibrary.org/obo/GAZ_00248016">
        <obo:RO_0001025 rdf:resource="http://purl.obolibrary.org/obo/GAZ_00051196"/>
        <obo:IAO_0000115>A semi-permanent saline lake.</obo:IAO_0000115>
        <oboInOwl:hasOBONamespace>GAZ</oboInOwl:hasOBONamespace>
        <oboInOwl:id>GAZ:00248016</oboInOwl:id>
        <rdfs:label>Lake Sitra</rdfs:label>
    </owl:NamedIndividual>
    


    <!-- http://purl.obolibrary.org/obo/GAZ_00248017 -->

    <owl:NamedIndividual rdf:about="http://purl.obolibrary.org/obo/GAZ_00248017">
        <obo:RO_0001025 rdf:resource="http://purl.obolibrary.org/obo/GAZ_00051196"/>
        <obo:IAO_0000115>A semi-permanent saline lake.</obo:IAO_0000115>
        <oboInOwl:hasOBONamespace>GAZ</oboInOwl:hasOBONamespace>
        <oboInOwl:id>GAZ:00248017</oboInOwl:id>
        <rdfs:label>Lake el Bahrein</rdfs:label>
    </owl:NamedIndividual>
    


    <!-- http://purl.obolibrary.org/obo/GAZ_00248018 -->

    <owl:NamedIndividual rdf:about="http://purl.obolibrary.org/obo/GAZ_00248018">
        <obo:RO_0001025 rdf:resource="http://purl.obolibrary.org/obo/GAZ_00051196"/>
        <obo:IAO_0000115>A semi-permanent saline lake.</obo:IAO_0000115>
        <oboInOwl:hasOBONamespace>GAZ</oboInOwl:hasOBONamespace>
        <oboInOwl:id>GAZ:00248018</oboInOwl:id>
        <rdfs:label>Lake el Maghra</rdfs:label>
    </owl:NamedIndividual>
    


    <!-- http://purl.obolibrary.org/obo/GAZ_00248111 -->

    <owl:NamedIndividual rdf:about="http://purl.obolibrary.org/obo/GAZ_00248111">
        <obo:RO_0001025 rdf:resource="http://purl.obolibrary.org/obo/GAZ_00002456"/>
        <obo:IAO_0000115>A bay.</obo:IAO_0000115>
        <oboInOwl:hasOBONamespace>GAZ</oboInOwl:hasOBONamespace>
        <oboInOwl:id>GAZ:00248111</oboInOwl:id>
        <rdfs:label>Mersa Mubarec</rdfs:label>
    </owl:NamedIndividual>
    


    <!-- http://purl.obolibrary.org/obo/GAZ_00248112 -->

    <owl:NamedIndividual rdf:about="http://purl.obolibrary.org/obo/GAZ_00248112">
        <obo:RO_0001025 rdf:resource="http://purl.obolibrary.org/obo/GAZ_00002456"/>
        <obo:IAO_0000115>An inlet.</obo:IAO_0000115>
        <oboInOwl:hasOBONamespace>GAZ</oboInOwl:hasOBONamespace>
        <oboInOwl:id>GAZ:00248112</oboInOwl:id>
        <rdfs:label>Mersa Deresa</rdfs:label>
    </owl:NamedIndividual>
    


    <!-- http://purl.obolibrary.org/obo/GAZ_00248117 -->

    <owl:NamedIndividual rdf:about="http://purl.obolibrary.org/obo/GAZ_00248117">
        <obo:RO_0001025 rdf:resource="http://purl.obolibrary.org/obo/GAZ_00002456"/>
        <obo:IAO_0000115>A bay.</obo:IAO_0000115>
        <oboInOwl:hasOBONamespace>GAZ</oboInOwl:hasOBONamespace>
        <oboInOwl:id>GAZ:00248117</oboInOwl:id>
        <rdfs:label>Assab Bahir Selat&apos;e</rdfs:label>
    </owl:NamedIndividual>
    


    <!-- http://purl.obolibrary.org/obo/GAZ_00248118 -->

    <owl:NamedIndividual rdf:about="http://purl.obolibrary.org/obo/GAZ_00248118">
        <obo:RO_0001025 rdf:resource="http://purl.obolibrary.org/obo/GAZ_00002456"/>
        <obo:RO_0001025 rdf:resource="http://purl.obolibrary.org/obo/GAZ_00248117"/>
        <obo:IAO_0000115>An island.</obo:IAO_0000115>
        <oboInOwl:hasOBONamespace>GAZ</oboInOwl:hasOBONamespace>
        <oboInOwl:id>GAZ:00248118</oboInOwl:id>
        <rdfs:label>Fatuma Deset</rdfs:label>
    </owl:NamedIndividual>
    


    <!-- http://purl.obolibrary.org/obo/GAZ_00251838 -->

    <owl:NamedIndividual rdf:about="http://purl.obolibrary.org/obo/GAZ_00251838">
        <obo:IAO_0000115>An erg.</obo:IAO_0000115>
        <oboInOwl:hasOBONamespace>GAZ</oboInOwl:hasOBONamespace>
        <oboInOwl:id>GAZ:00251838</oboInOwl:id>
        <rdfs:label>Idhan Ubari</rdfs:label>
    </owl:NamedIndividual>
    


    <!-- http://purl.obolibrary.org/obo/GAZ_00252194 -->

    <owl:NamedIndividual rdf:about="http://purl.obolibrary.org/obo/GAZ_00252194">
        <obo:RO_0001025 rdf:resource="http://purl.obolibrary.org/obo/GAZ_00252195"/>
        <obo:IAO_0000115>A guelta system.</obo:IAO_0000115>
        <oboInOwl:hasOBONamespace>GAZ</oboInOwl:hasOBONamespace>
        <oboInOwl:id>GAZ:00252194</oboInOwl:id>
        <rdfs:label>Gamra Ouarbi Gueltas</rdfs:label>
    </owl:NamedIndividual>
    


    <!-- http://purl.obolibrary.org/obo/GAZ_00252195 -->

    <owl:NamedIndividual rdf:about="http://purl.obolibrary.org/obo/GAZ_00252195">
        <obo:RO_0001025 rdf:resource="http://purl.obolibrary.org/obo/GAZ_00231580"/>
        <obo:IAO_0000115>A wadi.</obo:IAO_0000115>
        <oboInOwl:hasOBONamespace>GAZ</oboInOwl:hasOBONamespace>
        <oboInOwl:id>GAZ:00252195</oboInOwl:id>
        <rdfs:label>Oued Bourraga</rdfs:label>
    </owl:NamedIndividual>
    


    <!-- http://purl.obolibrary.org/obo/GAZ_00252196 -->

    <owl:NamedIndividual rdf:about="http://purl.obolibrary.org/obo/GAZ_00252196">
        <obo:RO_0001025 rdf:resource="http://purl.obolibrary.org/obo/GAZ_00252195"/>
        <obo:IAO_0000115>A spring.</obo:IAO_0000115>
        <oboInOwl:hasOBONamespace>GAZ</oboInOwl:hasOBONamespace>
        <oboInOwl:id>GAZ:00252196</oboInOwl:id>
        <rdfs:label>El Housseiniya</rdfs:label>
    </owl:NamedIndividual>
    


    <!-- http://purl.obolibrary.org/obo/GAZ_00252197 -->

    <owl:NamedIndividual rdf:about="http://purl.obolibrary.org/obo/GAZ_00252197">
        <obo:RO_0001025 rdf:resource="http://purl.obolibrary.org/obo/GAZ_00231580"/>
        <obo:IAO_0000115>An oasis. Located in the escarpment of the Tagant Plateau, in its southwestern extension towards Kiffa.</obo:IAO_0000115>
        <oboInOwl:hasOBONamespace>GAZ</oboInOwl:hasOBONamespace>
        <oboInOwl:id>GAZ:00252197</oboInOwl:id>
        <rdfs:label>Tartega Gueltas</rdfs:label>
    </owl:NamedIndividual>
    


    <!-- http://purl.obolibrary.org/obo/GAZ_00253017 -->

    <owl:NamedIndividual rdf:about="http://purl.obolibrary.org/obo/GAZ_00253017">
        <obo:RO_0001025 rdf:resource="http://purl.obolibrary.org/obo/GAZ_00103898"/>
        <obo:IAO_0000115>A wadi.</obo:IAO_0000115>
        <oboInOwl:hasOBONamespace>GAZ</oboInOwl:hasOBONamespace>
        <oboInOwl:id>GAZ:00253017</oboInOwl:id>
        <rdfs:label>Ighalabelabene</rdfs:label>
    </owl:NamedIndividual>
    


    <!-- http://purl.obolibrary.org/obo/GAZ_00253018 -->

    <owl:NamedIndividual rdf:about="http://purl.obolibrary.org/obo/GAZ_00253018">
        <obo:RO_0001025 rdf:resource="http://purl.obolibrary.org/obo/GAZ_00103898"/>
        <obo:IAO_0000115>A wadi.</obo:IAO_0000115>
        <oboInOwl:hasOBONamespace>GAZ</oboInOwl:hasOBONamespace>
        <oboInOwl:id>GAZ:00253018</oboInOwl:id>
        <rdfs:label>Nabarou</rdfs:label>
    </owl:NamedIndividual>
    


    <!-- http://purl.obolibrary.org/obo/GAZ_00253019 -->

    <owl:NamedIndividual rdf:about="http://purl.obolibrary.org/obo/GAZ_00253019">
        <obo:RO_0001025 rdf:resource="http://purl.obolibrary.org/obo/GAZ_00103898"/>
        <obo:IAO_0000115>A wadi.</obo:IAO_0000115>
        <oboInOwl:hasOBONamespace>GAZ</oboInOwl:hasOBONamespace>
        <oboInOwl:id>GAZ:00253019</oboInOwl:id>
        <rdfs:label>Bagzane-n-Ammas</rdfs:label>
    </owl:NamedIndividual>
    


    <!-- http://purl.obolibrary.org/obo/GAZ_00253020 -->

    <owl:NamedIndividual rdf:about="http://purl.obolibrary.org/obo/GAZ_00253020">
        <obo:RO_0001025 rdf:resource="http://purl.obolibrary.org/obo/GAZ_00103898"/>
        <obo:IAO_0000115>An intermittent river.</obo:IAO_0000115>
        <oboInOwl:hasOBONamespace>GAZ</oboInOwl:hasOBONamespace>
        <oboInOwl:id>GAZ:00253020</oboInOwl:id>
        <rdfs:label>Timia</rdfs:label>
    </owl:NamedIndividual>
    


    <!-- http://purl.obolibrary.org/obo/GAZ_00253021 -->

    <owl:NamedIndividual rdf:about="http://purl.obolibrary.org/obo/GAZ_00253021">
        <obo:RO_0001025 rdf:resource="http://purl.obolibrary.org/obo/GAZ_00103898"/>
        <obo:IAO_0000115>A wadi.</obo:IAO_0000115>
        <oboInOwl:hasOBONamespace>GAZ</oboInOwl:hasOBONamespace>
        <oboInOwl:id>GAZ:00253021</oboInOwl:id>
        <rdfs:label>Tamgak</rdfs:label>
    </owl:NamedIndividual>
    


    <!-- http://purl.obolibrary.org/obo/GAZ_00253022 -->

    <owl:NamedIndividual rdf:about="http://purl.obolibrary.org/obo/GAZ_00253022">
        <obo:RO_0001025 rdf:resource="http://purl.obolibrary.org/obo/GAZ_00103898"/>
        <obo:IAO_0000115>A plateau.</obo:IAO_0000115>
        <oboInOwl:hasOBONamespace>GAZ</oboInOwl:hasOBONamespace>
        <oboInOwl:id>GAZ:00253022</oboInOwl:id>
        <rdfs:label>Djado Massif</rdfs:label>
    </owl:NamedIndividual>
    


    <!-- http://purl.obolibrary.org/obo/GAZ_00253023 -->

    <owl:NamedIndividual rdf:about="http://purl.obolibrary.org/obo/GAZ_00253023">
        <obo:RO_0001025 rdf:resource="http://purl.obolibrary.org/obo/GAZ_00103898"/>
        <obo:IAO_0000115>A plateau.</obo:IAO_0000115>
        <oboInOwl:hasOBONamespace>GAZ</oboInOwl:hasOBONamespace>
        <oboInOwl:id>GAZ:00253023</oboInOwl:id>
        <rdfs:label>Kaquar Massif</rdfs:label>
    </owl:NamedIndividual>
    


    <!-- http://purl.obolibrary.org/obo/GAZ_00253024 -->

    <owl:NamedIndividual rdf:about="http://purl.obolibrary.org/obo/GAZ_00253024">
        <obo:RO_0001025 rdf:resource="http://purl.obolibrary.org/obo/GAZ_00103898"/>
        <obo:IAO_0000115>An escarpment.</obo:IAO_0000115>
        <oboInOwl:hasOBONamespace>GAZ</oboInOwl:hasOBONamespace>
        <oboInOwl:id>GAZ:00253024</oboInOwl:id>
        <rdfs:label>Fachi Massif</rdfs:label>
    </owl:NamedIndividual>
    


    <!-- http://purl.obolibrary.org/obo/GAZ_00256446 -->

    <owl:NamedIndividual rdf:about="http://purl.obolibrary.org/obo/GAZ_00256446">
        <obo:RO_0001025 rdf:resource="http://purl.obolibrary.org/obo/GAZ_00000654"/>
        <obo:RO_0001025 rdf:resource="http://purl.obolibrary.org/obo/GAZ_00176004"/>
        <obo:IAO_0000115>A group of islands off the coast of Africa, located in the Red Sea. The islands are located in the Halayeb Triangle, which is claimed by both Sudan and Egypt, as part of an ongoing border dispute. Since the 1990&apos;s, the are has been occupied by Egypt, and so the islands are de facto administered by Egypt.</obo:IAO_0000115>
        <oboInOwl:hasOBONamespace>GAZ</oboInOwl:hasOBONamespace>
        <oboInOwl:id>GAZ:00256446</oboInOwl:id>
        <rdfs:label>Siyal Islands</rdfs:label>
    </owl:NamedIndividual>
    


    <!-- http://purl.obolibrary.org/obo/GAZ_00256447 -->

    <owl:NamedIndividual rdf:about="http://purl.obolibrary.org/obo/GAZ_00256447">
        <obo:RO_0001025 rdf:resource="http://purl.obolibrary.org/obo/GAZ_00256446"/>
        <obo:IAO_0000115>An island.</obo:IAO_0000115>
        <oboInOwl:hasOBONamespace>GAZ</oboInOwl:hasOBONamespace>
        <oboInOwl:id>GAZ:00256447</oboInOwl:id>
        <rdfs:label>Siyal El Kabir</rdfs:label>
    </owl:NamedIndividual>
    


    <!-- http://purl.obolibrary.org/obo/GAZ_00256448 -->

    <owl:NamedIndividual rdf:about="http://purl.obolibrary.org/obo/GAZ_00256448">
        <obo:RO_0001025 rdf:resource="http://purl.obolibrary.org/obo/GAZ_00002456"/>
        <obo:IAO_0000115>A bay.</obo:IAO_0000115>
        <oboInOwl:hasOBONamespace>GAZ</oboInOwl:hasOBONamespace>
        <oboInOwl:id>GAZ:00256448</oboInOwl:id>
        <rdfs:label>Dungunab Bay</rdfs:label>
    </owl:NamedIndividual>
    


    <!-- http://purl.obolibrary.org/obo/GAZ_00256449 -->

    <owl:NamedIndividual rdf:about="http://purl.obolibrary.org/obo/GAZ_00256449">
        <obo:RO_0001025 rdf:resource="http://purl.obolibrary.org/obo/GAZ_00002456"/>
        <obo:IAO_0000115>An island.</obo:IAO_0000115>
        <oboInOwl:hasOBONamespace>GAZ</oboInOwl:hasOBONamespace>
        <oboInOwl:id>GAZ:00256449</oboInOwl:id>
        <rdfs:label>Jazirat Mukawwa&apos;</rdfs:label>
    </owl:NamedIndividual>
    


    <!-- http://purl.obolibrary.org/obo/GAZ_00256465 -->

    <owl:NamedIndividual rdf:about="http://purl.obolibrary.org/obo/GAZ_00256465">
        <obo:IAO_0000115>A river.</obo:IAO_0000115>
        <oboInOwl:hasOBONamespace>GAZ</oboInOwl:hasOBONamespace>
        <oboInOwl:id>GAZ:00256465</oboInOwl:id>
        <rdfs:label>Lileboak River</rdfs:label>
    </owl:NamedIndividual>
    


    <!-- http://purl.obolibrary.org/obo/GAZ_00256472 -->

    <owl:NamedIndividual rdf:about="http://purl.obolibrary.org/obo/GAZ_00256472">
        <obo:IAO_0000115>A dam.</obo:IAO_0000115>
        <oboInOwl:hasOBONamespace>GAZ</oboInOwl:hasOBONamespace>
        <oboInOwl:id>GAZ:00256472</oboInOwl:id>
        <rdfs:label>Jebel Auliya Dam</rdfs:label>
    </owl:NamedIndividual>
    


    <!-- http://purl.obolibrary.org/obo/GAZ_00256473 -->

    <owl:NamedIndividual rdf:about="http://purl.obolibrary.org/obo/GAZ_00256473">
        <obo:IAO_0000115>A reservoir. Impounded by Jebel Auliya Dam.</obo:IAO_0000115>
        <oboInOwl:hasOBONamespace>GAZ</oboInOwl:hasOBONamespace>
        <oboInOwl:id>GAZ:00256473</oboInOwl:id>
        <rdfs:label>Jebel Auliya Reservoir</rdfs:label>
    </owl:NamedIndividual>
    


    <!-- http://purl.obolibrary.org/obo/GAZ_00256482 -->

    <owl:NamedIndividual rdf:about="http://purl.obolibrary.org/obo/GAZ_00256482">
        <obo:IAO_0000115>An artificial lake. Impounded by El Roseires Dam.</obo:IAO_0000115>
        <oboInOwl:hasOBONamespace>GAZ</oboInOwl:hasOBONamespace>
        <oboInOwl:id>GAZ:00256482</oboInOwl:id>
        <rdfs:label>El Roseires Lake</rdfs:label>
    </owl:NamedIndividual>
    


    <!-- http://purl.obolibrary.org/obo/GAZ_00256483 -->

    <owl:NamedIndividual rdf:about="http://purl.obolibrary.org/obo/GAZ_00256483">
        <obo:IAO_0000115>An artifiical lake. Impounded by Sennar Dam.</obo:IAO_0000115>
        <oboInOwl:hasOBONamespace>GAZ</oboInOwl:hasOBONamespace>
        <oboInOwl:id>GAZ:00256483</oboInOwl:id>
        <rdfs:label>Sennar Lake</rdfs:label>
    </owl:NamedIndividual>
    


    <!-- http://purl.obolibrary.org/obo/GAZ_00256484 -->

    <owl:NamedIndividual rdf:about="http://purl.obolibrary.org/obo/GAZ_00256484">
        <obo:IAO_0000115>A dam. Impounds Kashim el Girlba Lake. Completed 1964.</obo:IAO_0000115>
        <oboInOwl:hasOBONamespace>GAZ</oboInOwl:hasOBONamespace>
        <oboInOwl:id>GAZ:00256484</oboInOwl:id>
        <rdfs:label>Kashim el Girlba Dam</rdfs:label>
    </owl:NamedIndividual>
    


    <!-- http://purl.obolibrary.org/obo/GAZ_00256485 -->

    <owl:NamedIndividual rdf:about="http://purl.obolibrary.org/obo/GAZ_00256485">
        <obo:IAO_0000115>An artifiical lake. Impounded by Kashim el Girlba Dam. Completed 1964.</obo:IAO_0000115>
        <oboInOwl:hasOBONamespace>GAZ</oboInOwl:hasOBONamespace>
        <oboInOwl:id>GAZ:00256485</oboInOwl:id>
        <rdfs:label>Kashim el Girlba Lake</rdfs:label>
    </owl:NamedIndividual>
    


    <!-- http://purl.obolibrary.org/obo/GAZ_00256486 -->

    <owl:NamedIndividual rdf:about="http://purl.obolibrary.org/obo/GAZ_00256486">
        <rdf:type rdf:resource="http://purl.obolibrary.org/obo/ENVO_00000074"/>
        <obo:IAO_0000115>A barrage. Located 25 km S of Khartoum.</obo:IAO_0000115>
        <oboInOwl:hasOBONamespace>GAZ</oboInOwl:hasOBONamespace>
        <oboInOwl:id>GAZ:00256486</oboInOwl:id>
        <rdfs:label>Gebel Auliya</rdfs:label>
    </owl:NamedIndividual>
    


    <!-- http://purl.obolibrary.org/obo/GAZ_00260292 -->

    <owl:NamedIndividual rdf:about="http://purl.obolibrary.org/obo/GAZ_00260292">
        <rdf:type rdf:resource="http://purl.obolibrary.org/obo/ENVO_00000475"/>
        <obo:RO_0001025 rdf:resource="http://purl.obolibrary.org/obo/GAZ_00058791"/>
        <obo:IAO_0000115>An arm of Lake Kyoga.</obo:IAO_0000115>
        <oboInOwl:hasOBONamespace>GAZ</oboInOwl:hasOBONamespace>
        <oboInOwl:id>GAZ:00260292</oboInOwl:id>
        <rdfs:label>Mpologoma Arm</rdfs:label>
    </owl:NamedIndividual>
    


    <!-- http://purl.obolibrary.org/obo/GAZ_00260861 -->

    <owl:NamedIndividual rdf:about="http://purl.obolibrary.org/obo/GAZ_00260861">
        <obo:RO_0001025 rdf:resource="http://purl.obolibrary.org/obo/GAZ_00002456"/>
        <obo:IAO_0000115>An island.</obo:IAO_0000115>
        <oboInOwl:hasOBONamespace>GAZ</oboInOwl:hasOBONamespace>
        <oboInOwl:id>GAZ:00260861</oboInOwl:id>
        <rdfs:label>Buhays Island</rdfs:label>
    </owl:NamedIndividual>
    


    <!-- http://purl.obolibrary.org/obo/GAZ_00260862 -->

    <owl:NamedIndividual rdf:about="http://purl.obolibrary.org/obo/GAZ_00260862">
        <obo:RO_0001025 rdf:resource="http://purl.obolibrary.org/obo/GAZ_00002456"/>
        <oboInOwl:hasOBONamespace>GAZ</oboInOwl:hasOBONamespace>
        <oboInOwl:id>GAZ:00260862</oboInOwl:id>
        <rdfs:label>Al-Badi Island</rdfs:label>
    </owl:NamedIndividual>
    


    <!-- http://purl.obolibrary.org/obo/GAZ_00260863 -->

    <owl:NamedIndividual rdf:about="http://purl.obolibrary.org/obo/GAZ_00260863">
        <obo:RO_0001025 rdf:resource="http://purl.obolibrary.org/obo/GAZ_00002456"/>
        <obo:IAO_0000115>An island.</obo:IAO_0000115>
        <oboInOwl:hasOBONamespace>GAZ</oboInOwl:hasOBONamespace>
        <oboInOwl:id>GAZ:00260863</oboInOwl:id>
        <rdfs:label>Tikfash Island</rdfs:label>
    </owl:NamedIndividual>
    


    <!-- http://purl.obolibrary.org/obo/GAZ_00260864 -->

    <owl:NamedIndividual rdf:about="http://purl.obolibrary.org/obo/GAZ_00260864">
        <obo:RO_0001025 rdf:resource="http://purl.obolibrary.org/obo/GAZ_00002456"/>
        <obo:IAO_0000115>An island.</obo:IAO_0000115>
        <oboInOwl:hasOBONamespace>GAZ</oboInOwl:hasOBONamespace>
        <oboInOwl:id>GAZ:00260864</oboInOwl:id>
        <rdfs:label>Humar Island</rdfs:label>
    </owl:NamedIndividual>
    


    <!-- http://purl.obolibrary.org/obo/GAZ_00260865 -->

    <owl:NamedIndividual rdf:about="http://purl.obolibrary.org/obo/GAZ_00260865">
        <obo:RO_0001025 rdf:resource="http://purl.obolibrary.org/obo/GAZ_00002456"/>
        <obo:IAO_0000115>An island.</obo:IAO_0000115>
        <oboInOwl:hasOBONamespace>GAZ</oboInOwl:hasOBONamespace>
        <oboInOwl:id>GAZ:00260865</oboInOwl:id>
        <rdfs:label>Kitamah Island</rdfs:label>
    </owl:NamedIndividual>
    


    <!-- http://purl.obolibrary.org/obo/GAZ_00260866 -->

    <owl:NamedIndividual rdf:about="http://purl.obolibrary.org/obo/GAZ_00260866">
        <obo:RO_0001025 rdf:resource="http://purl.obolibrary.org/obo/GAZ_00002456"/>
        <obo:IAO_0000115>An island.</obo:IAO_0000115>
        <oboInOwl:hasOBONamespace>GAZ</oboInOwl:hasOBONamespace>
        <oboInOwl:id>GAZ:00260866</oboInOwl:id>
        <rdfs:label>Zakhah Island</rdfs:label>
    </owl:NamedIndividual>
    


    <!-- http://purl.obolibrary.org/obo/GAZ_00260867 -->

    <owl:NamedIndividual rdf:about="http://purl.obolibrary.org/obo/GAZ_00260867">
        <obo:RO_0001025 rdf:resource="http://purl.obolibrary.org/obo/GAZ_00002456"/>
        <obo:IAO_0000115>An island.</obo:IAO_0000115>
        <oboInOwl:hasOBONamespace>GAZ</oboInOwl:hasOBONamespace>
        <oboInOwl:id>GAZ:00260867</oboInOwl:id>
        <rdfs:label>Zurbat Island</rdfs:label>
    </owl:NamedIndividual>
    


    <!-- http://purl.obolibrary.org/obo/GAZ_00260868 -->

    <owl:NamedIndividual rdf:about="http://purl.obolibrary.org/obo/GAZ_00260868">
        <obo:RO_0001025 rdf:resource="http://purl.obolibrary.org/obo/GAZ_00002456"/>
        <obo:IAO_0000115>An island.</obo:IAO_0000115>
        <oboInOwl:hasOBONamespace>GAZ</oboInOwl:hasOBONamespace>
        <oboInOwl:id>GAZ:00260868</oboInOwl:id>
        <rdfs:label>Juwa Island</rdfs:label>
    </owl:NamedIndividual>
    


    <!-- http://purl.obolibrary.org/obo/GAZ_00260869 -->

    <owl:NamedIndividual rdf:about="http://purl.obolibrary.org/obo/GAZ_00260869">
        <obo:RO_0001025 rdf:resource="http://purl.obolibrary.org/obo/GAZ_00002456"/>
        <obo:IAO_0000115>An island.</obo:IAO_0000115>
        <oboInOwl:hasOBONamespace>GAZ</oboInOwl:hasOBONamespace>
        <oboInOwl:id>GAZ:00260869</oboInOwl:id>
        <rdfs:label>At Talawin Island</rdfs:label>
    </owl:NamedIndividual>
    


    <!-- http://purl.obolibrary.org/obo/GAZ_00260871 -->

    <owl:NamedIndividual rdf:about="http://purl.obolibrary.org/obo/GAZ_00260871">
        <obo:RO_0001025 rdf:resource="http://purl.obolibrary.org/obo/GAZ_00002456"/>
        <obo:IAO_0000115>An island.</obo:IAO_0000115>
        <oboInOwl:hasOBONamespace>GAZ</oboInOwl:hasOBONamespace>
        <oboInOwl:id>GAZ:00260871</oboInOwl:id>
        <rdfs:label>Zabin Island</rdfs:label>
    </owl:NamedIndividual>
    


    <!-- http://purl.obolibrary.org/obo/GAZ_00260872 -->

    <owl:NamedIndividual rdf:about="http://purl.obolibrary.org/obo/GAZ_00260872">
        <obo:RO_0001025 rdf:resource="http://purl.obolibrary.org/obo/GAZ_00002456"/>
        <obo:IAO_0000115>An island.</obo:IAO_0000115>
        <oboInOwl:hasOBONamespace>GAZ</oboInOwl:hasOBONamespace>
        <oboInOwl:id>GAZ:00260872</oboInOwl:id>
        <rdfs:label>Al-Murk Island</rdfs:label>
    </owl:NamedIndividual>
    


    <!-- http://purl.obolibrary.org/obo/GAZ_00260873 -->

    <owl:NamedIndividual rdf:about="http://purl.obolibrary.org/obo/GAZ_00260873">
        <obo:RO_0001025 rdf:resource="http://purl.obolibrary.org/obo/GAZ_00002456"/>
        <obo:IAO_0000115>An island.</obo:IAO_0000115>
        <oboInOwl:hasOBONamespace>GAZ</oboInOwl:hasOBONamespace>
        <oboInOwl:id>GAZ:00260873</oboInOwl:id>
        <rdfs:label>Hataban Island</rdfs:label>
    </owl:NamedIndividual>
    


    <!-- http://purl.obolibrary.org/obo/GAZ_00260874 -->

    <owl:NamedIndividual rdf:about="http://purl.obolibrary.org/obo/GAZ_00260874">
        <obo:RO_0001025 rdf:resource="http://purl.obolibrary.org/obo/GAZ_00002456"/>
        <obo:IAO_0000115>An island.</obo:IAO_0000115>
        <oboInOwl:hasOBONamespace>GAZ</oboInOwl:hasOBONamespace>
        <oboInOwl:id>GAZ:00260874</oboInOwl:id>
        <rdfs:label>&apos;Ukban Island</rdfs:label>
    </owl:NamedIndividual>
    


    <!-- http://purl.obolibrary.org/obo/GAZ_00260875 -->

    <owl:NamedIndividual rdf:about="http://purl.obolibrary.org/obo/GAZ_00260875">
        <obo:RO_0001025 rdf:resource="http://purl.obolibrary.org/obo/GAZ_00002456"/>
        <obo:IAO_0000115>An island.</obo:IAO_0000115>
        <oboInOwl:hasOBONamespace>GAZ</oboInOwl:hasOBONamespace>
        <oboInOwl:id>GAZ:00260875</oboInOwl:id>
        <rdfs:label>Bahr Ibn Abbas</rdfs:label>
    </owl:NamedIndividual>
    


    <!-- http://purl.obolibrary.org/obo/GAZ_00281380 -->

    <owl:NamedIndividual rdf:about="http://purl.obolibrary.org/obo/GAZ_00281380">
        <obo:IAO_0000115>An island.</obo:IAO_0000115>
        <oboInOwl:hasOBONamespace>GAZ</oboInOwl:hasOBONamespace>
        <oboInOwl:id>GAZ:00281380</oboInOwl:id>
        <rdfs:label>Us Island</rdfs:label>
    </owl:NamedIndividual>
    


    <!-- http://purl.obolibrary.org/obo/GAZ_00281381 -->

    <owl:NamedIndividual rdf:about="http://purl.obolibrary.org/obo/GAZ_00281381">
        <obo:IAO_0000115>An island.</obo:IAO_0000115>
        <oboInOwl:hasOBONamespace>GAZ</oboInOwl:hasOBONamespace>
        <oboInOwl:id>GAZ:00281381</oboInOwl:id>
        <rdfs:label>Sur Island</rdfs:label>
    </owl:NamedIndividual>
    


    <!-- http://purl.obolibrary.org/obo/GAZ_00281382 -->

    <owl:NamedIndividual rdf:about="http://purl.obolibrary.org/obo/GAZ_00281382">
        <obo:IAO_0000115>An island.</obo:IAO_0000115>
        <oboInOwl:hasOBONamespace>GAZ</oboInOwl:hasOBONamespace>
        <oboInOwl:id>GAZ:00281382</oboInOwl:id>
        <rdfs:label>Sherari Island</rdfs:label>
    </owl:NamedIndividual>
    


    <!-- http://purl.obolibrary.org/obo/GAZ_00281422 -->

    <owl:NamedIndividual rdf:about="http://purl.obolibrary.org/obo/GAZ_00281422">
        <obo:IAO_0000115>A region in Libya known for extensive prehistoric rock art.</obo:IAO_0000115>
        <oboInOwl:hasOBONamespace>GAZ</oboInOwl:hasOBONamespace>
        <oboInOwl:id>GAZ:00281422</oboInOwl:id>
        <rdfs:label>Mesak Settafet</rdfs:label>
    </owl:NamedIndividual>
    


    <!-- http://purl.obolibrary.org/obo/GAZ_00281423 -->

    <owl:NamedIndividual rdf:about="http://purl.obolibrary.org/obo/GAZ_00281423">
        <obo:RO_0001025 rdf:resource="http://purl.obolibrary.org/obo/GAZ_00281422"/>
        <obo:IAO_0000115>A prehistoric archeological site in south western Libya in Mesak Settafet, famous for its rock engravings of different kinds.</obo:IAO_0000115>
        <oboInOwl:hasOBONamespace>GAZ</oboInOwl:hasOBONamespace>
        <oboInOwl:id>GAZ:00281423</oboInOwl:id>
        <rdfs:label>Wadi Mathendous</rdfs:label>
    </owl:NamedIndividual>
    


    <!-- http://purl.obolibrary.org/obo/GAZ_00281424 -->

    <owl:NamedIndividual rdf:about="http://purl.obolibrary.org/obo/GAZ_00281424">
        <obo:RO_0001025 rdf:resource="http://purl.obolibrary.org/obo/GAZ_00281422"/>
        <obo:IAO_0000115>A site of rock art.</obo:IAO_0000115>
        <oboInOwl:hasOBONamespace>GAZ</oboInOwl:hasOBONamespace>
        <oboInOwl:id>GAZ:00281424</oboInOwl:id>
        <rdfs:label>Ghalgiwan</rdfs:label>
    </owl:NamedIndividual>
    


    <!-- http://purl.obolibrary.org/obo/GAZ_00281425 -->

    <owl:NamedIndividual rdf:about="http://purl.obolibrary.org/obo/GAZ_00281425">
        <obo:RO_0001025 rdf:resource="http://purl.obolibrary.org/obo/GAZ_00281422"/>
        <obo:IAO_0000115>A site of rock art.</obo:IAO_0000115>
        <oboInOwl:hasOBONamespace>GAZ</oboInOwl:hasOBONamespace>
        <oboInOwl:id>GAZ:00281425</oboInOwl:id>
        <rdfs:label>Tiksaten</rdfs:label>
    </owl:NamedIndividual>
    


    <!-- http://purl.obolibrary.org/obo/GAZ_00281426 -->

    <owl:NamedIndividual rdf:about="http://purl.obolibrary.org/obo/GAZ_00281426">
        <obo:RO_0001025 rdf:resource="http://purl.obolibrary.org/obo/GAZ_00281422"/>
        <obo:IAO_0000115>A site of rock art.</obo:IAO_0000115>
        <oboInOwl:hasOBONamespace>GAZ</oboInOwl:hasOBONamespace>
        <oboInOwl:id>GAZ:00281426</oboInOwl:id>
        <rdfs:label>Abategh</rdfs:label>
    </owl:NamedIndividual>
    


    <!-- http://purl.obolibrary.org/obo/GAZ_00281428 -->

    <owl:NamedIndividual rdf:about="http://purl.obolibrary.org/obo/GAZ_00281428">
        <obo:RO_0001025 rdf:resource="http://purl.obolibrary.org/obo/GAZ_00000652"/>
        <obo:IAO_0000115>An archeological site. Located on Nile river, 50 miles NW of Thebes; was seat of first two Egyptian dynasties; was religious center for worship of Osiris in 4th dynasty; noted for ruined temples dating from reign of Ramses II (1292-1225 BC) &amp; Seti I (1313-1292 BC).</obo:IAO_0000115>
        <oboInOwl:hasOBONamespace>GAZ</oboInOwl:hasOBONamespace>
        <oboInOwl:id>GAZ:00281428</oboInOwl:id>
        <rdfs:label>Araba al-Madfuna</rdfs:label>
    </owl:NamedIndividual>
    


    <!-- 
    ///////////////////////////////////////////////////////////////////////////////////////
    //
    // Annotations
    //
    ///////////////////////////////////////////////////////////////////////////////////////
     -->

    <rdf:Description rdf:about="http://purl.obolibrary.org/obo/GAZ_00000645">
        <oboInOwl:hasOBONamespace>GAZ</oboInOwl:hasOBONamespace>
        <oboInOwl:id>GAZ:00000645</oboInOwl:id>
        <rdfs:label>Aswan Governorate</rdfs:label>
        <obo:IAO_0000115>One of the governorates of Egypt. It is the southmost governorate in Upper Egypt. The capital of the governorate is Aswan. It borders Qena Governorate to the north, Red Sea Governorate to the east, New Valley Governorate to the west, and Sudan to the south.</obo:IAO_0000115>
    </rdf:Description>
    <rdf:Description rdf:about="http://purl.obolibrary.org/obo/GAZ_00000646">
        <oboInOwl:hasOBONamespace>GAZ</oboInOwl:hasOBONamespace>
        <rdfs:label>Asyut Governorate</rdfs:label>
        <oboInOwl:id>GAZ:00000646</oboInOwl:id>
        <obo:IAO_0000115>One of the governorates of Egypt. It stretches for about 120 km along the banks of the Nile. The capital of the governorate is the city of Asyut.</obo:IAO_0000115>
    </rdf:Description>
    <rdf:Description rdf:about="http://purl.obolibrary.org/obo/GAZ_00000647">
        <rdfs:label>Beni Suef Governorate</rdfs:label>
        <obo:IAO_0000115>One of the governorates of Egypt. It is in the centre of the country.</obo:IAO_0000115>
        <oboInOwl:hasOBONamespace>GAZ</oboInOwl:hasOBONamespace>
        <oboInOwl:id>GAZ:00000647</oboInOwl:id>
    </rdf:Description>
    <rdf:Description rdf:about="http://purl.obolibrary.org/obo/GAZ_00000648">
        <rdfs:label>Faiyum Governorate</rdfs:label>
        <obo:IAO_0000115>One of the governorates of Egypt located in the middle of the country.</obo:IAO_0000115>
        <oboInOwl:hasOBONamespace>GAZ</oboInOwl:hasOBONamespace>
        <oboInOwl:id>GAZ:00000648</oboInOwl:id>
    </rdf:Description>
    <rdf:Description rdf:about="http://purl.obolibrary.org/obo/GAZ_00000649">
        <rdfs:label>Giza Governorate</rdfs:label>
        <oboInOwl:id>GAZ:00000649</oboInOwl:id>
        <obo:IAO_0000115>One of the governorates of Egypt. It is in the center of the country.</obo:IAO_0000115>
        <oboInOwl:hasOBONamespace>GAZ</oboInOwl:hasOBONamespace>
    </rdf:Description>
    <rdf:Description rdf:about="http://purl.obolibrary.org/obo/GAZ_00000650">
        <oboInOwl:hasOBONamespace>GAZ</oboInOwl:hasOBONamespace>
        <oboInOwl:id>GAZ:00000650</oboInOwl:id>
        <rdfs:label>Minya Governorate</rdfs:label>
        <obo:IAO_0000115>One of the governorates of Upper Egypt.</obo:IAO_0000115>
    </rdf:Description>
    <rdf:Description rdf:about="http://purl.obolibrary.org/obo/GAZ_00000651">
        <obo:IAO_0000115>One of the governorates of Egypt. It is in the south of the country, and covers a stretch of the Nile valley. Its capital is the city of Qena.</obo:IAO_0000115>
        <rdfs:label>Qena Governorate</rdfs:label>
        <oboInOwl:id>GAZ:00000651</oboInOwl:id>
        <oboInOwl:hasOBONamespace>GAZ</oboInOwl:hasOBONamespace>
    </rdf:Description>
    <rdf:Description rdf:about="http://purl.obolibrary.org/obo/GAZ_00000652">
        <oboInOwl:id>GAZ:00000652</oboInOwl:id>
        <rdfs:label>Sohag Governorate</rdfs:label>
        <oboInOwl:hasOBONamespace>GAZ</oboInOwl:hasOBONamespace>
        <obo:IAO_0000115>One of the governorates of Egypt. It is in the south of the country (Upper Egypt), and covers a stretch of the Nile Valley. Its capital is the city of Sohag.</obo:IAO_0000115>
    </rdf:Description>
    <rdf:Description rdf:about="http://purl.obolibrary.org/obo/GAZ_00000653">
        <obo:IAO_0000115>One of the governorates of Egypt, located in the north of the country, lying directly on the Mediterranean Sea.</obo:IAO_0000115>
        <rdfs:label>Alexandria Governorate</rdfs:label>
        <oboInOwl:id>GAZ:00000653</oboInOwl:id>
        <oboInOwl:hasOBONamespace>GAZ</oboInOwl:hasOBONamespace>
    </rdf:Description>
    <rdf:Description rdf:about="http://purl.obolibrary.org/obo/GAZ_00000654">
        <oboInOwl:id>GAZ:00000654</oboInOwl:id>
        <rdfs:label>Red Sea Governorate</rdfs:label>
        <obo:IAO_0000115>One of the governorates of Egypt. It is located between the Nile and the Red Sea in the southeast of the country and its southern border forms part of Egypt&apos;s border with Sudan. Its capital is Hurghada.</obo:IAO_0000115>
        <oboInOwl:hasOBONamespace>GAZ</oboInOwl:hasOBONamespace>
    </rdf:Description>
    <rdf:Description rdf:about="http://purl.obolibrary.org/obo/GAZ_00000655">
        <oboInOwl:id>GAZ:00000655</oboInOwl:id>
        <rdfs:label>Beheira Governorate</rdfs:label>
        <oboInOwl:hasOBONamespace>GAZ</oboInOwl:hasOBONamespace>
        <obo:IAO_0000115>One of the governorates of Egypt. It is in the north of the country.</obo:IAO_0000115>
    </rdf:Description>
    <rdf:Description rdf:about="http://purl.obolibrary.org/obo/GAZ_00000656">
        <obo:IAO_0000115>One of the governorates of Egypt, lying northeast of Cairo.</obo:IAO_0000115>
        <rdfs:label>Dakahlia Governorate</rdfs:label>
        <oboInOwl:id>GAZ:00000656</oboInOwl:id>
        <oboInOwl:hasOBONamespace>GAZ</oboInOwl:hasOBONamespace>
    </rdf:Description>
    <rdf:Description rdf:about="http://purl.obolibrary.org/obo/GAZ_00000657">
        <rdfs:label>Damietta Governorate</rdfs:label>
        <obo:IAO_0000115>One of the governorates of Egypt. It is in the north of the country.</obo:IAO_0000115>
        <oboInOwl:id>GAZ:00000657</oboInOwl:id>
        <oboInOwl:hasOBONamespace>GAZ</oboInOwl:hasOBONamespace>
    </rdf:Description>
    <rdf:Description rdf:about="http://purl.obolibrary.org/obo/GAZ_00000658">
        <obo:IAO_0000115>One of the governorates of Egypt. It is located in the north of the country, south of Kafr el-Sheikh Governorate, and north of Monufia Governorate. Its capital is Tanta.</obo:IAO_0000115>
        <rdfs:label>Gharbia Governorate</rdfs:label>
        <oboInOwl:hasOBONamespace>GAZ</oboInOwl:hasOBONamespace>
        <oboInOwl:id>GAZ:00000658</oboInOwl:id>
    </rdf:Description>
    <rdf:Description rdf:about="http://purl.obolibrary.org/obo/GAZ_00000659">
        <obo:IAO_0000115>One of the governorates of Egypt. It lies in the north of the country along the western branch of the Nile. Its capital is the city of Kafr el-Sheikh. It was once part of the Gharbia Governorate.</obo:IAO_0000115>
        <rdfs:label>Kafr el-Sheikh Governorate</rdfs:label>
        <oboInOwl:id>GAZ:00000659</oboInOwl:id>
        <oboInOwl:hasOBONamespace>GAZ</oboInOwl:hasOBONamespace>
    </rdf:Description>
    <rdf:Description rdf:about="http://purl.obolibrary.org/obo/GAZ_00000660">
        <rdfs:label>Monufia Governorate</rdfs:label>
        <oboInOwl:hasOBONamespace>GAZ</oboInOwl:hasOBONamespace>
        <oboInOwl:id>GAZ:00000660</oboInOwl:id>
        <obo:IAO_0000115>One of the governorates of Egypt. It is in the north of the country (south of Gharbiyah and north of Cairo) and its capital is Shibin el-Kom.</obo:IAO_0000115>
    </rdf:Description>
    <rdf:Description rdf:about="http://purl.obolibrary.org/obo/GAZ_00000661">
        <obo:IAO_0000115>One of the governorates of Egypt. It is in the north of the country. Its capital is Banha.</obo:IAO_0000115>
        <rdfs:label>Qalyubia Governorate</rdfs:label>
        <oboInOwl:id>GAZ:00000661</oboInOwl:id>
        <oboInOwl:hasOBONamespace>GAZ</oboInOwl:hasOBONamespace>
    </rdf:Description>
    <rdf:Description rdf:about="http://purl.obolibrary.org/obo/GAZ_00000662">
        <obo:IAO_0000115>One of the governorates of Egypt. It is in the north of the country. Its capital is Zagazig.</obo:IAO_0000115>
        <rdfs:label>Sharqia Governorate</rdfs:label>
        <oboInOwl:id>GAZ:00000662</oboInOwl:id>
        <oboInOwl:hasOBONamespace>GAZ</oboInOwl:hasOBONamespace>
    </rdf:Description>
    <rdf:Description rdf:about="http://purl.obolibrary.org/obo/GAZ_00000663">
        <oboInOwl:id>GAZ:00000663</oboInOwl:id>
        <oboInOwl:hasOBONamespace>GAZ</oboInOwl:hasOBONamespace>
        <obo:IAO_0000115>One of the governorates of Egypt. Its capital is the national capital of Cairo.</obo:IAO_0000115>
        <rdfs:label>Cairo Governorate</rdfs:label>
    </rdf:Description>
    <rdf:Description rdf:about="http://purl.obolibrary.org/obo/GAZ_00000664">
        <obo:IAO_0000115>One of the governorates of Egypt. It is in the northeast of the country. Its capital is the city of Ismailia.</obo:IAO_0000115>
        <oboInOwl:hasOBONamespace>GAZ</oboInOwl:hasOBONamespace>
        <oboInOwl:id>GAZ:00000664</oboInOwl:id>
        <rdfs:label>Ismailia Governorate</rdfs:label>
    </rdf:Description>
    <rdf:Description rdf:about="http://purl.obolibrary.org/obo/GAZ_00000665">
        <obo:IAO_0000115>One of the governorates of Egypt. It is in the northeast of the country. Its capital is the city of Port Said.</obo:IAO_0000115>
        <oboInOwl:id>GAZ:00000665</oboInOwl:id>
        <oboInOwl:hasOBONamespace>GAZ</oboInOwl:hasOBONamespace>
        <rdfs:label>Port Said Governorate</rdfs:label>
    </rdf:Description>
    <rdf:Description rdf:about="http://purl.obolibrary.org/obo/GAZ_00000666">
        <obo:IAO_0000115>One of the governorates of Egypt. It is in the northeast of the country and is coterminous with the city of Suez. It is situated East of Delta, North of Suez Gulf.</obo:IAO_0000115>
        <oboInOwl:id>GAZ:00000666</oboInOwl:id>
        <oboInOwl:hasOBONamespace>GAZ</oboInOwl:hasOBONamespace>
        <rdfs:label>Suez Governorate</rdfs:label>
    </rdf:Description>
    <rdf:Description rdf:about="http://purl.obolibrary.org/obo/GAZ_00000667">
        <obo:IAO_0000115>One of the governorates of Egypt. It is in the north-west of the country, bordering Libya. Its capital is Mersa Matruh.</obo:IAO_0000115>
        <oboInOwl:hasOBONamespace>GAZ</oboInOwl:hasOBONamespace>
        <rdfs:label>Matruh Governorate</rdfs:label>
        <oboInOwl:id>GAZ:00000667</oboInOwl:id>
    </rdf:Description>
    <rdf:Description rdf:about="http://purl.obolibrary.org/obo/GAZ_00000668">
        <obo:IAO_0000115>One of the governorates of Egypt. It is in the south-west of the country, between the Nile and Libya. Its capital is the Kharga Oasis.</obo:IAO_0000115>
        <rdfs:label>New Valley Governorate</rdfs:label>
        <oboInOwl:hasOBONamespace>GAZ</oboInOwl:hasOBONamespace>
        <oboInOwl:id>GAZ:00000668</oboInOwl:id>
    </rdf:Description>
    <rdf:Description rdf:about="http://purl.obolibrary.org/obo/GAZ_00003933">
        <oboInOwl:id>GAZ:00003933</oboInOwl:id>
        <oboInOwl:hasOBONamespace>GAZ</oboInOwl:hasOBONamespace>
        <rdfs:label>Governorate (Egypt in Africa)</rdfs:label>
    </rdf:Description>
    <rdf:Description rdf:about="http://purl.obolibrary.org/obo/GAZ_00003934">
        <oboInOwl:id>GAZ:00003934</oboInOwl:id>
        <oboInOwl:hasOBONamespace>GAZ</oboInOwl:hasOBONamespace>
        <obo:IAO_0000115>A country in North Africa that includes the Sinai Peninsula, a land bridge to Asia. Egypt borders Libya to the west, Sudan to the south, and the Gaza Strip and Israel to the east. The northern coast borders the Mediterranean Sea and the island of Cyprus; the eastern coast borders the Red Sea. Egypt is divided into 26 governorates (in Arabic, called muhafazat, singular muhafazah). The governorates are further divided into regions (markazes).</obo:IAO_0000115>
        <rdfs:label>Egypt</rdfs:label>
    </rdf:Description>
    <rdf:Description rdf:about="http://purl.obolibrary.org/obo/GAZ_00005648">
        <oboInOwl:hasOBONamespace>GAZ</oboInOwl:hasOBONamespace>
        <oboInOwl:id>GAZ:00005648</oboInOwl:id>
        <rdfs:label>Cairo</rdfs:label>
    </rdf:Description>
    <rdf:Description rdf:about="http://purl.obolibrary.org/obo/GAZ_00005649">
        <oboInOwl:hasOBONamespace>GAZ</oboInOwl:hasOBONamespace>
        <oboInOwl:id>GAZ:00005649</oboInOwl:id>
        <rdfs:label>populated place, Egypt</rdfs:label>
    </rdf:Description>
    <rdf:Description rdf:about="http://purl.obolibrary.org/obo/GAZ_00012404">
        <rdfs:label>Ismailia</rdfs:label>
        <obo:IAO_0000115>The capital of Al Isma&apos;iliyah Governorate. It is located on the west bank of the Suez Canal, approximately half way between Port Said to the north and Suez to the south. The Canal widens at that point to include Timsah, one of the Bitter Lakes linked by the Canal.</obo:IAO_0000115>
        <oboInOwl:hasOBONamespace>GAZ</oboInOwl:hasOBONamespace>
        <oboInOwl:id>GAZ:00012404</oboInOwl:id>
    </rdf:Description>
    <rdf:Description rdf:about="http://purl.obolibrary.org/obo/GAZ_00052491">
        <rdfs:label>Alexandria</rdfs:label>
        <oboInOwl:hasOBONamespace>GAZ</oboInOwl:hasOBONamespace>
        <obo:IAO_0000115>A city that extends about 32 km along the coast of the Mediterranean sea in north-central Egypt. Modern Alexandria is divided into 6 hais (urban districts).</obo:IAO_0000115>
        <oboInOwl:id>GAZ:00052491</oboInOwl:id>
    </rdf:Description>
    <rdf:Description rdf:about="http://purl.obolibrary.org/obo/GAZ_00052492">
        <oboInOwl:hasOBONamespace>GAZ</oboInOwl:hasOBONamespace>
        <rdfs:label>Aswan</rdfs:label>
        <obo:IAO_0000115>A populated place. A city in the south of Egypt, the capital of the Aswan Governorate. It stands on the east bank of the Nile at the first cataract.</obo:IAO_0000115>
        <oboInOwl:id>GAZ:00052492</oboInOwl:id>
    </rdf:Description>
    <rdf:Description rdf:about="http://purl.obolibrary.org/obo/GAZ_00052493">
        <oboInOwl:hasOBONamespace>GAZ</oboInOwl:hasOBONamespace>
        <obo:IAO_0000115>A populated place. located on the west bank of the Nile River between Esna and Aswan.</obo:IAO_0000115>
        <rdfs:label>Edfou</rdfs:label>
        <oboInOwl:id>GAZ:00052493</oboInOwl:id>
    </rdf:Description>
    <rdf:Description rdf:about="http://purl.obolibrary.org/obo/GAZ_00058884">
        <oboInOwl:id>GAZ:00058884</oboInOwl:id>
        <obo:IAO_0000115>Shallow stretches between Aswan and Khartoum where the water&apos;s surface is broken by numerous small boulders and stones lying on the river bed, as well as many small rocky islets. In some places, these stretches are punctuated by whitewater and are perhaps well characterized as rapids, while in others the water flow is smoother.</obo:IAO_0000115>
        <oboInOwl:hasOBONamespace>GAZ</oboInOwl:hasOBONamespace>
        <rdfs:label>Cataracts of the Nile</rdfs:label>
    </rdf:Description>
    <rdf:Description rdf:about="http://purl.obolibrary.org/obo/GAZ_00058886">
        <oboInOwl:id>GAZ:00058886</oboInOwl:id>
        <obo:IAO_0000115>A cataract on the River Nile in the Manasir Desert, Sudan. It will be flooded by the Merowe Dam from 2006.</obo:IAO_0000115>
        <rdfs:label>Fourth Cataract</rdfs:label>
        <oboInOwl:hasOBONamespace>GAZ</oboInOwl:hasOBONamespace>
    </rdf:Description>
    <rdf:Description rdf:about="http://purl.obolibrary.org/obo/GAZ_00058890">
        <rdfs:label>First Cataract</rdfs:label>
        <obo:IAO_0000115>A cataract on the River Nile near Aswan.</obo:IAO_0000115>
        <oboInOwl:hasOBONamespace>GAZ</oboInOwl:hasOBONamespace>
        <oboInOwl:id>GAZ:00058890</oboInOwl:id>
    </rdf:Description>
    <rdf:Description rdf:about="http://purl.obolibrary.org/obo/GAZ_00066400">
        <rdfs:label>Luxor Governorate</rdfs:label>
        <oboInOwl:id>GAZ:00066400</oboInOwl:id>
        <oboInOwl:hasOBONamespace>GAZ</oboInOwl:hasOBONamespace>
        <obo:IAO_0000115>One of the governorates of Egypt. It is in the south of the country along the Nile. Its capital is Luxor.</obo:IAO_0000115>
    </rdf:Description>
    <rdf:Description rdf:about="http://purl.obolibrary.org/obo/GAZ_00089771">
        <rdfs:label>Maadi</rdfs:label>
        <oboInOwl:hasOBONamespace>GAZ</oboInOwl:hasOBONamespace>
        <obo:IAO_0000115>A suburb south of Cairo, Egypt.</obo:IAO_0000115>
        <oboInOwl:id>GAZ:00089771</oboInOwl:id>
    </rdf:Description>
    <rdf:Description rdf:about="http://purl.obolibrary.org/obo/GAZ_00230304">
        <rdfs:label>Helwan Governorate</rdfs:label>
        <oboInOwl:hasOBONamespace>GAZ</oboInOwl:hasOBONamespace>
        <oboInOwl:id>GAZ:00230304</oboInOwl:id>
        <obo:IAO_0000115>One of the governorates of Egypt. It is in the north of the country (Lower Egypt), and covers a stretch of the Nile Valley. In 2008-04, parts of the administrative division of the Cairo governorate was split into two, Cairo and Helwan, with Helwan encompassing most of the suburbs of Cairo, new compounds and rural southern villages. Helwan became the capital of the new Helwan governorate.</obo:IAO_0000115>
    </rdf:Description>
    <rdf:Description rdf:about="http://purl.obolibrary.org/obo/GAZ_00230305">
        <oboInOwl:id>GAZ:00230305</oboInOwl:id>
        <obo:IAO_0000115>One of the governorates of Egypt. It is in the north of the country (Lower Egypt), it is located west of the Nile Valley. It was formerly a part of the Giza Governorate, but it was declared a separate governorate in 2008-04.</obo:IAO_0000115>
        <oboInOwl:hasOBONamespace>GAZ</oboInOwl:hasOBONamespace>
        <rdfs:label>6th of October Governorate</rdfs:label>
    </rdf:Description>
</rdf:RDF>



<!-- Generated by the OWL API (version 4.5.6) https://github.com/owlcs/owlapi -->

