<?xml version="1.0"?>
<rdf:RDF xmlns="http://purl.obolibrary.org/obo/gaz/subsets/countries/Eritrea.owl#"
     xml:base="http://purl.obolibrary.org/obo/gaz/subsets/countries/Eritrea.owl"
     xmlns:obo="http://purl.obolibrary.org/obo/"
     xmlns:owl="http://www.w3.org/2002/07/owl#"
     xmlns:rdf="http://www.w3.org/1999/02/22-rdf-syntax-ns#"
     xmlns:xml="http://www.w3.org/XML/1998/namespace"
     xmlns:xsd="http://www.w3.org/2001/XMLSchema#"
     xmlns:rdfs="http://www.w3.org/2000/01/rdf-schema#"
     xmlns:oboInOwl="http://www.geneontology.org/formats/oboInOwl#">
    <owl:Ontology rdf:about="http://purl.obolibrary.org/obo/gaz/subsets/countries/Eritrea.owl">
        <owl:imports rdf:resource="http://purl.obolibrary.org/obo/gaz/imports/envo_import.owl"/>
        <owl:imports rdf:resource="http://purl.obolibrary.org/obo/gaz/imports/ro_import.owl"/>
    </owl:Ontology>
    


    <!-- 
    ///////////////////////////////////////////////////////////////////////////////////////
    //
    // Annotation properties
    //
    ///////////////////////////////////////////////////////////////////////////////////////
     -->

    


    <!-- http://purl.obolibrary.org/obo/IAO_0000115 -->

    <owl:AnnotationProperty rdf:about="http://purl.obolibrary.org/obo/IAO_0000115"/>
    


    <!-- http://www.geneontology.org/formats/oboInOwl#hasOBONamespace -->

    <owl:AnnotationProperty rdf:about="http://www.geneontology.org/formats/oboInOwl#hasOBONamespace"/>
    


    <!-- http://www.geneontology.org/formats/oboInOwl#id -->

    <owl:AnnotationProperty rdf:about="http://www.geneontology.org/formats/oboInOwl#id"/>
    


    <!-- 
    ///////////////////////////////////////////////////////////////////////////////////////
    //
    // Object Properties
    //
    ///////////////////////////////////////////////////////////////////////////////////////
     -->

    


    <!-- http://purl.obolibrary.org/obo/RO_0001025 -->

    <owl:ObjectProperty rdf:about="http://purl.obolibrary.org/obo/RO_0001025"/>
    


    <!-- 
    ///////////////////////////////////////////////////////////////////////////////////////
    //
    // Classes
    //
    ///////////////////////////////////////////////////////////////////////////////////////
     -->

    


    <!-- http://purl.obolibrary.org/obo/ENVO_00000004 -->

    <owl:Class rdf:about="http://purl.obolibrary.org/obo/ENVO_00000004"/>
    


    <!-- http://purl.obolibrary.org/obo/ENVO_00000019 -->

    <owl:Class rdf:about="http://purl.obolibrary.org/obo/ENVO_00000019"/>
    


    <!-- http://purl.obolibrary.org/obo/ENVO_00000032 -->

    <owl:Class rdf:about="http://purl.obolibrary.org/obo/ENVO_00000032"/>
    


    <!-- http://purl.obolibrary.org/obo/ENVO_00000100 -->

    <owl:Class rdf:about="http://purl.obolibrary.org/obo/ENVO_00000100"/>
    


    <!-- http://purl.obolibrary.org/obo/ENVO_00000106 -->

    <owl:Class rdf:about="http://purl.obolibrary.org/obo/ENVO_00000106"/>
    


    <!-- http://purl.obolibrary.org/obo/ENVO_00000191 -->

    <owl:Class rdf:about="http://purl.obolibrary.org/obo/ENVO_00000191"/>
    


    <!-- http://purl.obolibrary.org/obo/ENVO_00000220 -->

    <owl:Class rdf:about="http://purl.obolibrary.org/obo/ENVO_00000220"/>
    


    <!-- http://purl.obolibrary.org/obo/ENVO_00000309 -->

    <owl:Class rdf:about="http://purl.obolibrary.org/obo/ENVO_00000309"/>
    


    <!-- http://purl.obolibrary.org/obo/ENVO_00000354 -->

    <owl:Class rdf:about="http://purl.obolibrary.org/obo/ENVO_00000354"/>
    


    <!-- http://purl.obolibrary.org/obo/ENVO_00000475 -->

    <owl:Class rdf:about="http://purl.obolibrary.org/obo/ENVO_00000475"/>
    


    <!-- http://purl.obolibrary.org/obo/ENVO_00000479 -->

    <owl:Class rdf:about="http://purl.obolibrary.org/obo/ENVO_00000479"/>
    


    <!-- http://purl.obolibrary.org/obo/ENVO_00000856 -->

    <owl:Class rdf:about="http://purl.obolibrary.org/obo/ENVO_00000856"/>
    


    <!-- http://purl.obolibrary.org/obo/GAZ_00000771 -->

    <owl:Class rdf:about="http://purl.obolibrary.org/obo/GAZ_00000771"/>
    


    <!-- http://purl.obolibrary.org/obo/GAZ_00000772 -->

    <owl:Class rdf:about="http://purl.obolibrary.org/obo/GAZ_00000772">
        <rdfs:subClassOf rdf:resource="http://purl.obolibrary.org/obo/GAZ_00000771"/>
    </owl:Class>
    


    <!-- http://purl.obolibrary.org/obo/GAZ_00000773 -->

    <owl:Class rdf:about="http://purl.obolibrary.org/obo/GAZ_00000773">
        <rdfs:subClassOf rdf:resource="http://purl.obolibrary.org/obo/GAZ_00000771"/>
    </owl:Class>
    


    <!-- http://purl.obolibrary.org/obo/GAZ_00000774 -->

    <owl:Class rdf:about="http://purl.obolibrary.org/obo/GAZ_00000774">
        <rdfs:subClassOf rdf:resource="http://purl.obolibrary.org/obo/GAZ_00000771"/>
    </owl:Class>
    


    <!-- http://purl.obolibrary.org/obo/GAZ_00000776 -->

    <owl:Class rdf:about="http://purl.obolibrary.org/obo/GAZ_00000776">
        <rdfs:subClassOf rdf:resource="http://purl.obolibrary.org/obo/GAZ_00000771"/>
    </owl:Class>
    


    <!-- http://purl.obolibrary.org/obo/GAZ_00000777 -->

    <owl:Class rdf:about="http://purl.obolibrary.org/obo/GAZ_00000777">
        <rdfs:subClassOf rdf:resource="http://purl.obolibrary.org/obo/GAZ_00000771"/>
    </owl:Class>
    


    <!-- http://purl.obolibrary.org/obo/GAZ_10000775 -->

    <owl:Class rdf:about="http://purl.obolibrary.org/obo/GAZ_10000775">
        <rdfs:subClassOf rdf:resource="http://purl.obolibrary.org/obo/GAZ_00000771"/>
    </owl:Class>
    


    <!-- 
    ///////////////////////////////////////////////////////////////////////////////////////
    //
    // Individuals
    //
    ///////////////////////////////////////////////////////////////////////////////////////
     -->

    


    <!-- http://purl.obolibrary.org/obo/GAZ_00000007 -->

    <owl:NamedIndividual rdf:about="http://purl.obolibrary.org/obo/GAZ_00000007">
        <obo:IAO_0000115>A rift valley. A geographical and geological feature, approximately 6,000 km in length, that runs from northern Syria in Southwest Asia to central Mozambique in East Africa.</obo:IAO_0000115>
        <oboInOwl:hasOBONamespace>GAZ</oboInOwl:hasOBONamespace>
        <oboInOwl:id>GAZ:00000007</oboInOwl:id>
        <rdfs:label>Great Rift Valley</rdfs:label>
    </owl:NamedIndividual>
    


    <!-- http://purl.obolibrary.org/obo/GAZ_00000008 -->

    <owl:NamedIndividual rdf:about="http://purl.obolibrary.org/obo/GAZ_00000008">
        <obo:RO_0001025 rdf:resource="http://purl.obolibrary.org/obo/GAZ_00000007"/>
        <obo:IAO_0000115>A soda lake, in the eastern part of the Great Rift Valley. A Ramsar Site.</obo:IAO_0000115>
        <oboInOwl:hasOBONamespace>GAZ</oboInOwl:hasOBONamespace>
        <oboInOwl:id>GAZ:00000008</oboInOwl:id>
        <rdfs:label>Lake Elmenteita</rdfs:label>
    </owl:NamedIndividual>
    


    <!-- http://purl.obolibrary.org/obo/GAZ_00000058 -->

    <owl:NamedIndividual rdf:about="http://purl.obolibrary.org/obo/GAZ_00000058">
        <obo:RO_0001025 rdf:resource="http://purl.obolibrary.org/obo/GAZ_00000007"/>
        <obo:IAO_0000115>A freshwater lake that is the most southerly lake in the Great African Rift Valley system. Its largest tributary is the Ruhuhu and its outlet is the Shire River, a tributary of the Zambezi.</obo:IAO_0000115>
        <oboInOwl:hasOBONamespace>GAZ</oboInOwl:hasOBONamespace>
        <oboInOwl:id>GAZ:00000058</oboInOwl:id>
        <rdfs:label>Lake Malawi</rdfs:label>
    </owl:NamedIndividual>
    


    <!-- http://purl.obolibrary.org/obo/GAZ_00000581 -->

    <owl:NamedIndividual rdf:about="http://purl.obolibrary.org/obo/GAZ_00000581">
        <obo:IAO_0000115>A country situated in northern East Africa. It is bordered by Sudan in the west, Ethiopia in the south, and Djibouti in the southeast. The east and northeast of the country have an extensive coastline on the Red Sea, directly across from Saudi Arabia and Yemen. The Dahlak Archipelago and several of the Hanish Islands are part of Eritrea. Eritrea is divided into six regions (zobas) and subdivided into districts (&quot;sub-zobas&quot;).</obo:IAO_0000115>
        <oboInOwl:hasOBONamespace>GAZ</oboInOwl:hasOBONamespace>
        <oboInOwl:id>GAZ:00000581</oboInOwl:id>
        <rdfs:label>Eritrea</rdfs:label>
    </owl:NamedIndividual>
    


    <!-- http://purl.obolibrary.org/obo/GAZ_00000771 -->

    <owl:NamedIndividual rdf:about="http://purl.obolibrary.org/obo/GAZ_00000771">
        <obo:RO_0001025 rdf:resource="http://purl.obolibrary.org/obo/GAZ_00000581"/>
    </owl:NamedIndividual>
    


    <!-- http://purl.obolibrary.org/obo/GAZ_00000772 -->

    <owl:NamedIndividual rdf:about="http://purl.obolibrary.org/obo/GAZ_00000772"/>
    


    <!-- http://purl.obolibrary.org/obo/GAZ_00000773 -->

    <owl:NamedIndividual rdf:about="http://purl.obolibrary.org/obo/GAZ_00000773"/>
    


    <!-- http://purl.obolibrary.org/obo/GAZ_00000774 -->

    <owl:NamedIndividual rdf:about="http://purl.obolibrary.org/obo/GAZ_00000774"/>
    


    <!-- http://purl.obolibrary.org/obo/GAZ_00000776 -->

    <owl:NamedIndividual rdf:about="http://purl.obolibrary.org/obo/GAZ_00000776"/>
    


    <!-- http://purl.obolibrary.org/obo/GAZ_00000777 -->

    <owl:NamedIndividual rdf:about="http://purl.obolibrary.org/obo/GAZ_00000777"/>
    


    <!-- http://purl.obolibrary.org/obo/GAZ_00002477 -->

    <owl:NamedIndividual rdf:about="http://purl.obolibrary.org/obo/GAZ_00002477">
        <obo:RO_0001025 rdf:resource="http://purl.obolibrary.org/obo/GAZ_00007520"/>
        <obo:IAO_0000115>A saline lake between the West Bank and Israel to the west, and Jordan to the east.</obo:IAO_0000115>
        <oboInOwl:hasOBONamespace>GAZ</oboInOwl:hasOBONamespace>
        <oboInOwl:id>GAZ:00002477</oboInOwl:id>
        <rdfs:label>Dead Sea</rdfs:label>
    </owl:NamedIndividual>
    


    <!-- http://purl.obolibrary.org/obo/GAZ_00007520 -->

    <owl:NamedIndividual rdf:about="http://purl.obolibrary.org/obo/GAZ_00007520">
        <obo:RO_0001025 rdf:resource="http://purl.obolibrary.org/obo/GAZ_00044915"/>
        <obo:IAO_0000115>A river in Southwest Asia flowing through the Great Rift Valley into the Dead Sea.</obo:IAO_0000115>
        <oboInOwl:hasOBONamespace>GAZ</oboInOwl:hasOBONamespace>
        <oboInOwl:id>GAZ:00007520</oboInOwl:id>
        <rdfs:label>River Jordan</rdfs:label>
    </owl:NamedIndividual>
    


    <!-- http://purl.obolibrary.org/obo/GAZ_00007523 -->

    <owl:NamedIndividual rdf:about="http://purl.obolibrary.org/obo/GAZ_00007523">
        <obo:RO_0001025 rdf:resource="http://purl.obolibrary.org/obo/GAZ_00000007"/>
        <obo:IAO_0000115>A saline, alkaline lake, approximately 100 km2 in size, that lies in a graben. The lake is an example of a &quot;saline pan&quot;. The lake water, which is a dense sodium carbonate brine, precipitates vast quanitites of the mineral called trona (sodium sesquicarbonate). In places, the salt is up to 40 m thick. The lake is recharged mainly by saline hot springs (temperatures up to about 83degC) that discharge into alkaline &quot;lagoons&quot; around the lake margins, there being little surface runoff in this arid region. Most hot springs lie along the northwestern and southern shorelines of the lake. During the rainy season a thin (&lt;1m) layer of brine covers much of the saline pan, but this evaporates rapidly leaving a vast expanse of white salt that cracks to produce large polygons.</obo:IAO_0000115>
        <oboInOwl:hasOBONamespace>GAZ</oboInOwl:hasOBONamespace>
        <oboInOwl:id>GAZ:00007523</oboInOwl:id>
        <rdfs:label>Lake Magadi</rdfs:label>
    </owl:NamedIndividual>
    


    <!-- http://purl.obolibrary.org/obo/GAZ_00007862 -->

    <owl:NamedIndividual rdf:about="http://purl.obolibrary.org/obo/GAZ_00007862">
        <rdf:type rdf:resource="http://purl.obolibrary.org/obo/ENVO_00000032"/>
        <obo:RO_0001025 rdf:resource="http://purl.obolibrary.org/obo/GAZ_00000007"/>
        <obo:IAO_0000115>A gulf situated northeastward and adjacent to the Red Sea, bounded by the coasts of Sinai Peninsula and Arabian Peninsula. Its southern limit with the Red Sea (in the Strait of T Degrees r Degrees n) is the following: A line joining Cape Al Qa Degrees bah (28 Degrees 01430 Seconds N - 34 Degrees 37 Minutes 15 Seconds E), in Saudi Arabia, southwestward to position 27 Degrees 58 Minutes 10 Seconds N - 34 Degrees 35 Minutes E) on the coast of T Degrees r Degrees n Island; thence from this position southward, through T Degrees r Degrees n Island, to its southwestern extremity (27 Degrees 54 Minutes 50 Seconds N - 34 Degrees 33 Minutes E); and thence from the southwestern extremity of T Degrees r Degrees n Island westward, along the parallel of 27 Degrees 54 Minutes 50 Seconds N, to the coast of Sinai Peninsula, in Egypt.</obo:IAO_0000115>
        <oboInOwl:hasOBONamespace>GAZ</oboInOwl:hasOBONamespace>
        <oboInOwl:id>GAZ:00007862</oboInOwl:id>
        <rdfs:label>Gulf of Aqaba</rdfs:label>
    </owl:NamedIndividual>
    


    <!-- http://purl.obolibrary.org/obo/GAZ_00008411 -->

    <owl:NamedIndividual rdf:about="http://purl.obolibrary.org/obo/GAZ_00008411">
        <obo:RO_0001025 rdf:resource="http://purl.obolibrary.org/obo/GAZ_00000007"/>
        <obo:IAO_0000115>A saline, alkaline lake that lies in a volcanic region in a half-graben basin south of Lake Baringo, Kenya, a little north of the equator. A Ramsar Site.</obo:IAO_0000115>
        <oboInOwl:hasOBONamespace>GAZ</oboInOwl:hasOBONamespace>
        <oboInOwl:id>GAZ:00008411</oboInOwl:id>
        <rdfs:label>Lake Bogoria</rdfs:label>
    </owl:NamedIndividual>
    


    <!-- http://purl.obolibrary.org/obo/GAZ_00008558 -->

    <owl:NamedIndividual rdf:about="http://purl.obolibrary.org/obo/GAZ_00008558">
        <obo:RO_0001025 rdf:resource="http://purl.obolibrary.org/obo/GAZ_00000007"/>
        <obo:IAO_0000115>A meromictic lake that on the border between the Democratic Republic of the Congo and Rwanda, and is in the Albertine (western) Rift, a part of the Great Rift Valley. Lake Kivu empties into the Ruzizi River, which flows southwards into Lake Tanganyika.</obo:IAO_0000115>
        <oboInOwl:hasOBONamespace>GAZ</oboInOwl:hasOBONamespace>
        <oboInOwl:id>GAZ:00008558</oboInOwl:id>
        <rdfs:label>Lake Kivu</rdfs:label>
    </owl:NamedIndividual>
    


    <!-- http://purl.obolibrary.org/obo/GAZ_00008742 -->

    <owl:NamedIndividual rdf:about="http://purl.obolibrary.org/obo/GAZ_00008742">
        <obo:RO_0001025 rdf:resource="http://purl.obolibrary.org/obo/GAZ_00044915"/>
        <obo:IAO_0000115>A valley that lies within the northern part of the Syrian-African Rift Valley at an elevation of about 70 m above sea level. On both sides of the valley are steep slopes -- the Golan Heights to the east and the Upper Galilee mountains to the west, rise to 400 to 900 m above sea level. Basaltic hills of about 200 m above sea level along the southern side of the valley intercept the Jordan River, and are commonly referred to as the basalt &quot;plug&quot; (actually a temporary geologic base level), as they restrict water drainage downstream into the Sea of Galilee (Lake Kinneret). The Hula Valley covers an area of 177 km2 (25 km by 6-8 km.</obo:IAO_0000115>
        <oboInOwl:hasOBONamespace>GAZ</oboInOwl:hasOBONamespace>
        <oboInOwl:id>GAZ:00008742</oboInOwl:id>
        <rdfs:label>Hulah Valley</rdfs:label>
    </owl:NamedIndividual>
    


    <!-- http://purl.obolibrary.org/obo/GAZ_00008743 -->

    <owl:NamedIndividual rdf:about="http://purl.obolibrary.org/obo/GAZ_00008743">
        <obo:RO_0001025 rdf:resource="http://purl.obolibrary.org/obo/GAZ_00193886"/>
        <obo:IAO_0000115>A wetland.</obo:IAO_0000115>
        <oboInOwl:hasOBONamespace>GAZ</oboInOwl:hasOBONamespace>
        <oboInOwl:id>GAZ:00008743</oboInOwl:id>
        <rdfs:label>Hulah Swamp</rdfs:label>
    </owl:NamedIndividual>
    


    <!-- http://purl.obolibrary.org/obo/GAZ_00009142 -->

    <owl:NamedIndividual rdf:about="http://purl.obolibrary.org/obo/GAZ_00009142">
        <obo:RO_0001025 rdf:resource="http://purl.obolibrary.org/obo/GAZ_00008558"/>
        <obo:IAO_0000115>An island in Lake Kivu, belonging to the Democratic Republic of the Congo. At 40 km in length and with an area of 285 km2.</obo:IAO_0000115>
        <oboInOwl:hasOBONamespace>GAZ</oboInOwl:hasOBONamespace>
        <oboInOwl:id>GAZ:00009142</oboInOwl:id>
        <rdfs:label>Idjwi Island</rdfs:label>
    </owl:NamedIndividual>
    


    <!-- http://purl.obolibrary.org/obo/GAZ_00009683 -->

    <owl:NamedIndividual rdf:about="http://purl.obolibrary.org/obo/GAZ_00009683">
        <rdf:type rdf:resource="http://purl.obolibrary.org/obo/ENVO_00000220"/>
        <obo:RO_0001025 rdf:resource="http://purl.obolibrary.org/obo/GAZ_00000777"/>
        <obo:RO_0001025 rdf:resource="http://purl.obolibrary.org/obo/GAZ_00076365"/>
        <obo:IAO_0000115>An island group located in the Red Sea near Massawa, Eritrea. It consists of two large and 124 small islands.</obo:IAO_0000115>
        <oboInOwl:hasOBONamespace>GAZ</oboInOwl:hasOBONamespace>
        <oboInOwl:id>GAZ:00009683</oboInOwl:id>
        <rdfs:label>Dahlak Archipelago</rdfs:label>
    </owl:NamedIndividual>
    


    <!-- http://purl.obolibrary.org/obo/GAZ_00010533 -->

    <owl:NamedIndividual rdf:about="http://purl.obolibrary.org/obo/GAZ_00010533">
        <obo:RO_0001025 rdf:resource="http://purl.obolibrary.org/obo/GAZ_00044915"/>
        <obo:IAO_0000115>A large fertile plain and inland valley in the south of the Lower Galilee region of Israel. It is bordered to the south by the Samaria highlands and Mount Gilboa, to the north by the Lower Galilee, to the west by the Mount Carmel range, and to the east by the Jordan Valley.</obo:IAO_0000115>
        <oboInOwl:hasOBONamespace>GAZ</oboInOwl:hasOBONamespace>
        <oboInOwl:id>GAZ:00010533</oboInOwl:id>
        <rdfs:label>Jezreel Valley</rdfs:label>
    </owl:NamedIndividual>
    


    <!-- http://purl.obolibrary.org/obo/GAZ_00011722 -->

    <owl:NamedIndividual rdf:about="http://purl.obolibrary.org/obo/GAZ_00011722">
        <obo:RO_0001025 rdf:resource="http://purl.obolibrary.org/obo/GAZ_00000007"/>
        <obo:IAO_0000115>A freshwater lake is situated within the Western Rift of the Great Rift Valley. The major inflows are the Ruzizi River, entering the north of the lake from Lake Kivu, and the Malagarasi River, which is Tanzania&apos;s second largest river, entering in the east side of Lake Tanganyika. The Malagarasi pre-dates Lake Tanganyika and was formerly continuous with the Congo river.</obo:IAO_0000115>
        <oboInOwl:hasOBONamespace>GAZ</oboInOwl:hasOBONamespace>
        <oboInOwl:id>GAZ:00011722</oboInOwl:id>
        <rdfs:label>Lake Tanganyika</rdfs:label>
    </owl:NamedIndividual>
    


    <!-- http://purl.obolibrary.org/obo/GAZ_00015452 -->

    <owl:NamedIndividual rdf:about="http://purl.obolibrary.org/obo/GAZ_00015452">
        <obo:RO_0001025 rdf:resource="http://purl.obolibrary.org/obo/GAZ_00000007"/>
        <obo:IAO_0000115>A very large monictic freshwater lake bordering Kenya, Tanzania and Uganda.</obo:IAO_0000115>
        <oboInOwl:hasOBONamespace>GAZ</oboInOwl:hasOBONamespace>
        <oboInOwl:id>GAZ:00015452</oboInOwl:id>
        <rdfs:label>Lake Victoria</rdfs:label>
    </owl:NamedIndividual>
    


    <!-- http://purl.obolibrary.org/obo/GAZ_00015453 -->

    <owl:NamedIndividual rdf:about="http://purl.obolibrary.org/obo/GAZ_00015453">
        <obo:RO_0001025 rdf:resource="http://purl.obolibrary.org/obo/GAZ_00124567"/>
        <obo:IAO_0000115>A chain of more than fifty smaller islands, a few km off the northern shore of Lake Victoria, Uganda in the Napoleon Gulf.</obo:IAO_0000115>
        <oboInOwl:hasOBONamespace>GAZ</oboInOwl:hasOBONamespace>
        <oboInOwl:id>GAZ:00015453</oboInOwl:id>
        <rdfs:label>Buvuma Islands</rdfs:label>
    </owl:NamedIndividual>
    


    <!-- http://purl.obolibrary.org/obo/GAZ_00029996 -->

    <owl:NamedIndividual rdf:about="http://purl.obolibrary.org/obo/GAZ_00029996">
        <obo:RO_0001025 rdf:resource="http://purl.obolibrary.org/obo/GAZ_00000058"/>
        <obo:IAO_0000115>The smaller of two inhabited islands in Lake Malawi. It lies just a few km from Mozambique, and is entirely surrounded by Mozambican territorial waters, but belongs to Malawi.It is, therefore, an exclave of Malawi.</obo:IAO_0000115>
        <oboInOwl:hasOBONamespace>GAZ</oboInOwl:hasOBONamespace>
        <oboInOwl:id>GAZ:00029996</oboInOwl:id>
        <rdfs:label>Chisumulu Island</rdfs:label>
    </owl:NamedIndividual>
    


    <!-- http://purl.obolibrary.org/obo/GAZ_00029997 -->

    <owl:NamedIndividual rdf:about="http://purl.obolibrary.org/obo/GAZ_00029997">
        <obo:RO_0001025 rdf:resource="http://purl.obolibrary.org/obo/GAZ_00000058"/>
        <obo:IAO_0000115>The larger of two inhabited islands in Lake Malawi. It lies just a few km from Mozambique, and is surrounded by Mozambican territorial waters, but belongs to Malawi. An exclave of Malawi.</obo:IAO_0000115>
        <oboInOwl:hasOBONamespace>GAZ</oboInOwl:hasOBONamespace>
        <oboInOwl:id>GAZ:00029997</oboInOwl:id>
        <rdfs:label>Likoma Island</rdfs:label>
    </owl:NamedIndividual>
    


    <!-- http://purl.obolibrary.org/obo/GAZ_00031035 -->

    <owl:NamedIndividual rdf:about="http://purl.obolibrary.org/obo/GAZ_00031035">
        <rdf:type rdf:resource="http://purl.obolibrary.org/obo/ENVO_00000004"/>
        <obo:RO_0001025 rdf:resource="http://purl.obolibrary.org/obo/GAZ_00000772"/>
        <obo:IAO_0000115>A district in the Anseba region of northern Eritrea. The capital lies at Halhal.</obo:IAO_0000115>
        <oboInOwl:hasOBONamespace>GAZ</oboInOwl:hasOBONamespace>
        <oboInOwl:id>GAZ:00031035</oboInOwl:id>
        <rdfs:label>Halhal District</rdfs:label>
    </owl:NamedIndividual>
    


    <!-- http://purl.obolibrary.org/obo/GAZ_00031036 -->

    <owl:NamedIndividual rdf:about="http://purl.obolibrary.org/obo/GAZ_00031036">
        <rdf:type rdf:resource="http://purl.obolibrary.org/obo/ENVO_00000004"/>
        <obo:RO_0001025 rdf:resource="http://purl.obolibrary.org/obo/GAZ_00000772"/>
        <obo:IAO_0000115>A district in the Anseba region of northern Eritrea. The capital lies at Habero.</obo:IAO_0000115>
        <oboInOwl:hasOBONamespace>GAZ</oboInOwl:hasOBONamespace>
        <oboInOwl:id>GAZ:00031036</oboInOwl:id>
        <rdfs:label>Habero District</rdfs:label>
    </owl:NamedIndividual>
    


    <!-- http://purl.obolibrary.org/obo/GAZ_00031037 -->

    <owl:NamedIndividual rdf:about="http://purl.obolibrary.org/obo/GAZ_00031037">
        <rdf:type rdf:resource="http://purl.obolibrary.org/obo/ENVO_00000004"/>
        <obo:RO_0001025 rdf:resource="http://purl.obolibrary.org/obo/GAZ_00000772"/>
        <obo:IAO_0000115>A district in the Anseba region of northern Eritrea. The capital lies at Elabered.</obo:IAO_0000115>
        <oboInOwl:hasOBONamespace>GAZ</oboInOwl:hasOBONamespace>
        <oboInOwl:id>GAZ:00031037</oboInOwl:id>
        <rdfs:label>Elabered District</rdfs:label>
    </owl:NamedIndividual>
    


    <!-- http://purl.obolibrary.org/obo/GAZ_00031038 -->

    <owl:NamedIndividual rdf:about="http://purl.obolibrary.org/obo/GAZ_00031038">
        <rdf:type rdf:resource="http://purl.obolibrary.org/obo/ENVO_00000004"/>
        <obo:RO_0001025 rdf:resource="http://purl.obolibrary.org/obo/GAZ_00000772"/>
        <obo:IAO_0000115>A district in the Anseba region of northern Eritrea. The capital lies at Sela.</obo:IAO_0000115>
        <oboInOwl:hasOBONamespace>GAZ</oboInOwl:hasOBONamespace>
        <oboInOwl:id>GAZ:00031038</oboInOwl:id>
        <rdfs:label>Sela District</rdfs:label>
    </owl:NamedIndividual>
    


    <!-- http://purl.obolibrary.org/obo/GAZ_00031039 -->

    <owl:NamedIndividual rdf:about="http://purl.obolibrary.org/obo/GAZ_00031039">
        <rdf:type rdf:resource="http://purl.obolibrary.org/obo/ENVO_00000004"/>
        <obo:RO_0001025 rdf:resource="http://purl.obolibrary.org/obo/GAZ_00000772"/>
        <obo:IAO_0000115>A district in the Anseba region of northern Eritrea. The capital lies at Hagaz.</obo:IAO_0000115>
        <oboInOwl:hasOBONamespace>GAZ</oboInOwl:hasOBONamespace>
        <oboInOwl:id>GAZ:00031039</oboInOwl:id>
        <rdfs:label>Hagaz District</rdfs:label>
    </owl:NamedIndividual>
    


    <!-- http://purl.obolibrary.org/obo/GAZ_00031040 -->

    <owl:NamedIndividual rdf:about="http://purl.obolibrary.org/obo/GAZ_00031040">
        <obo:RO_0001025 rdf:resource="http://purl.obolibrary.org/obo/GAZ_00230329"/>
        <obo:IAO_0000115>The second largest city in Eritrea, lying north west of Asmara.</obo:IAO_0000115>
        <oboInOwl:hasOBONamespace>GAZ</oboInOwl:hasOBONamespace>
        <oboInOwl:id>GAZ:00031040</oboInOwl:id>
        <rdfs:label>Keren City</rdfs:label>
    </owl:NamedIndividual>
    


    <!-- http://purl.obolibrary.org/obo/GAZ_00031041 -->

    <owl:NamedIndividual rdf:about="http://purl.obolibrary.org/obo/GAZ_00031041">
        <rdf:type rdf:resource="http://purl.obolibrary.org/obo/ENVO_00000004"/>
        <obo:RO_0001025 rdf:resource="http://purl.obolibrary.org/obo/GAZ_00000772"/>
        <obo:IAO_0000115>A district in the Anseba region of northern Eritrea. The capital lies at Asmat.</obo:IAO_0000115>
        <oboInOwl:hasOBONamespace>GAZ</oboInOwl:hasOBONamespace>
        <oboInOwl:id>GAZ:00031041</oboInOwl:id>
        <rdfs:label>Asmat District</rdfs:label>
    </owl:NamedIndividual>
    


    <!-- http://purl.obolibrary.org/obo/GAZ_00031042 -->

    <owl:NamedIndividual rdf:about="http://purl.obolibrary.org/obo/GAZ_00031042">
        <rdf:type rdf:resource="http://purl.obolibrary.org/obo/ENVO_00000004"/>
        <obo:RO_0001025 rdf:resource="http://purl.obolibrary.org/obo/GAZ_00000772"/>
        <obo:IAO_0000115>A district in the Anseba region of northern Eritrea. The capital lies at Geleb.</obo:IAO_0000115>
        <oboInOwl:hasOBONamespace>GAZ</oboInOwl:hasOBONamespace>
        <oboInOwl:id>GAZ:00031042</oboInOwl:id>
        <rdfs:label>Geleb District</rdfs:label>
    </owl:NamedIndividual>
    


    <!-- http://purl.obolibrary.org/obo/GAZ_00031043 -->

    <owl:NamedIndividual rdf:about="http://purl.obolibrary.org/obo/GAZ_00031043">
        <rdf:type rdf:resource="http://purl.obolibrary.org/obo/ENVO_00000004"/>
        <obo:RO_0001025 rdf:resource="http://purl.obolibrary.org/obo/GAZ_00000772"/>
        <obo:IAO_0000115>A district in the Anseba region of northern Eritrea. The capital lies at Kerkebet.</obo:IAO_0000115>
        <oboInOwl:hasOBONamespace>GAZ</oboInOwl:hasOBONamespace>
        <oboInOwl:id>GAZ:00031043</oboInOwl:id>
        <rdfs:label>Kerkebet District</rdfs:label>
    </owl:NamedIndividual>
    


    <!-- http://purl.obolibrary.org/obo/GAZ_00031044 -->

    <owl:NamedIndividual rdf:about="http://purl.obolibrary.org/obo/GAZ_00031044">
        <rdf:type rdf:resource="http://purl.obolibrary.org/obo/ENVO_00000004"/>
        <obo:RO_0001025 rdf:resource="http://purl.obolibrary.org/obo/GAZ_00000773"/>
        <obo:IAO_0000115>A district in the Central Region of central Eritrea. The capital lies at Serejaka.</obo:IAO_0000115>
        <oboInOwl:hasOBONamespace>GAZ</oboInOwl:hasOBONamespace>
        <oboInOwl:id>GAZ:00031044</oboInOwl:id>
        <rdfs:label>Serejaka District</rdfs:label>
    </owl:NamedIndividual>
    


    <!-- http://purl.obolibrary.org/obo/GAZ_00031045 -->

    <owl:NamedIndividual rdf:about="http://purl.obolibrary.org/obo/GAZ_00031045">
        <rdf:type rdf:resource="http://purl.obolibrary.org/obo/ENVO_00000004"/>
        <obo:RO_0001025 rdf:resource="http://purl.obolibrary.org/obo/GAZ_00000773"/>
        <obo:IAO_0000115>A district in the Central Region of central Eritrea. The capital lies at Ghala Nefhi.</obo:IAO_0000115>
        <oboInOwl:hasOBONamespace>GAZ</oboInOwl:hasOBONamespace>
        <oboInOwl:id>GAZ:00031045</oboInOwl:id>
        <rdfs:label>Ghala Nefhi District</rdfs:label>
    </owl:NamedIndividual>
    


    <!-- http://purl.obolibrary.org/obo/GAZ_00031046 -->

    <owl:NamedIndividual rdf:about="http://purl.obolibrary.org/obo/GAZ_00031046">
        <rdf:type rdf:resource="http://purl.obolibrary.org/obo/ENVO_00000004"/>
        <obo:RO_0001025 rdf:resource="http://purl.obolibrary.org/obo/GAZ_00000773"/>
        <obo:IAO_0000115>A district in the Central Region of central Eritrea.</obo:IAO_0000115>
        <oboInOwl:hasOBONamespace>GAZ</oboInOwl:hasOBONamespace>
        <oboInOwl:id>GAZ:00031046</oboInOwl:id>
        <rdfs:label>South Western District</rdfs:label>
    </owl:NamedIndividual>
    


    <!-- http://purl.obolibrary.org/obo/GAZ_00031047 -->

    <owl:NamedIndividual rdf:about="http://purl.obolibrary.org/obo/GAZ_00031047">
        <rdf:type rdf:resource="http://purl.obolibrary.org/obo/ENVO_00000004"/>
        <obo:RO_0001025 rdf:resource="http://purl.obolibrary.org/obo/GAZ_00000773"/>
        <obo:IAO_0000115>A district in the Central Region of central Eritrea. The capital lies at Berikh.</obo:IAO_0000115>
        <oboInOwl:hasOBONamespace>GAZ</oboInOwl:hasOBONamespace>
        <oboInOwl:id>GAZ:00031047</oboInOwl:id>
        <rdfs:label>Berikh District</rdfs:label>
    </owl:NamedIndividual>
    


    <!-- http://purl.obolibrary.org/obo/GAZ_00031048 -->

    <owl:NamedIndividual rdf:about="http://purl.obolibrary.org/obo/GAZ_00031048">
        <rdf:type rdf:resource="http://purl.obolibrary.org/obo/ENVO_00000004"/>
        <obo:RO_0001025 rdf:resource="http://purl.obolibrary.org/obo/GAZ_00000773"/>
        <obo:IAO_0000115>A district in the Central Region of central Eritrea.</obo:IAO_0000115>
        <oboInOwl:hasOBONamespace>GAZ</oboInOwl:hasOBONamespace>
        <oboInOwl:id>GAZ:00031048</oboInOwl:id>
        <rdfs:label>North Eastern District</rdfs:label>
    </owl:NamedIndividual>
    


    <!-- http://purl.obolibrary.org/obo/GAZ_00031049 -->

    <owl:NamedIndividual rdf:about="http://purl.obolibrary.org/obo/GAZ_00031049">
        <rdf:type rdf:resource="http://purl.obolibrary.org/obo/ENVO_00000004"/>
        <obo:RO_0001025 rdf:resource="http://purl.obolibrary.org/obo/GAZ_00000773"/>
        <obo:IAO_0000115>A district in the Central Region of central Eritrea.</obo:IAO_0000115>
        <oboInOwl:hasOBONamespace>GAZ</oboInOwl:hasOBONamespace>
        <oboInOwl:id>GAZ:00031049</oboInOwl:id>
        <rdfs:label>South Eastern District</rdfs:label>
    </owl:NamedIndividual>
    


    <!-- http://purl.obolibrary.org/obo/GAZ_00031050 -->

    <owl:NamedIndividual rdf:about="http://purl.obolibrary.org/obo/GAZ_00031050">
        <rdf:type rdf:resource="http://purl.obolibrary.org/obo/ENVO_00000004"/>
        <obo:RO_0001025 rdf:resource="http://purl.obolibrary.org/obo/GAZ_00000774"/>
        <obo:IAO_0000115>A district in the Gash-Barka region of western Eritrea. The capital lies at Haykota.</obo:IAO_0000115>
        <oboInOwl:hasOBONamespace>GAZ</oboInOwl:hasOBONamespace>
        <oboInOwl:id>GAZ:00031050</oboInOwl:id>
        <rdfs:label>Haykota District</rdfs:label>
    </owl:NamedIndividual>
    


    <!-- http://purl.obolibrary.org/obo/GAZ_00031051 -->

    <owl:NamedIndividual rdf:about="http://purl.obolibrary.org/obo/GAZ_00031051">
        <rdf:type rdf:resource="http://purl.obolibrary.org/obo/ENVO_00000004"/>
        <obo:RO_0001025 rdf:resource="http://purl.obolibrary.org/obo/GAZ_00000774"/>
        <obo:IAO_0000115>A district in the Gash-Barka region of western Eritrea. The capital lies at Mensura.</obo:IAO_0000115>
        <oboInOwl:hasOBONamespace>GAZ</oboInOwl:hasOBONamespace>
        <oboInOwl:id>GAZ:00031051</oboInOwl:id>
        <rdfs:label>Mensura District</rdfs:label>
    </owl:NamedIndividual>
    


    <!-- http://purl.obolibrary.org/obo/GAZ_00031052 -->

    <owl:NamedIndividual rdf:about="http://purl.obolibrary.org/obo/GAZ_00031052">
        <rdf:type rdf:resource="http://purl.obolibrary.org/obo/ENVO_00000004"/>
        <obo:RO_0001025 rdf:resource="http://purl.obolibrary.org/obo/GAZ_00000774"/>
        <obo:IAO_0000115>A district in the Gash-Barka region of western Eritrea. The capital lies at Forto.</obo:IAO_0000115>
        <oboInOwl:hasOBONamespace>GAZ</oboInOwl:hasOBONamespace>
        <oboInOwl:id>GAZ:00031052</oboInOwl:id>
        <rdfs:label>Forto District</rdfs:label>
    </owl:NamedIndividual>
    


    <!-- http://purl.obolibrary.org/obo/GAZ_00031053 -->

    <owl:NamedIndividual rdf:about="http://purl.obolibrary.org/obo/GAZ_00031053">
        <rdf:type rdf:resource="http://purl.obolibrary.org/obo/ENVO_00000004"/>
        <obo:RO_0001025 rdf:resource="http://purl.obolibrary.org/obo/GAZ_00000774"/>
        <obo:IAO_0000115>A district in the Gash-Barka region of western Eritrea. The capital lies at Logo Anseba.</obo:IAO_0000115>
        <oboInOwl:hasOBONamespace>GAZ</oboInOwl:hasOBONamespace>
        <oboInOwl:id>GAZ:00031053</oboInOwl:id>
        <rdfs:label>Logo Anseba District</rdfs:label>
    </owl:NamedIndividual>
    


    <!-- http://purl.obolibrary.org/obo/GAZ_00031054 -->

    <owl:NamedIndividual rdf:about="http://purl.obolibrary.org/obo/GAZ_00031054">
        <rdf:type rdf:resource="http://purl.obolibrary.org/obo/ENVO_00000004"/>
        <obo:RO_0001025 rdf:resource="http://purl.obolibrary.org/obo/GAZ_00000774"/>
        <obo:IAO_0000115>A district in the Gash-Barka region of western Eritrea. The capital lies at Gogne.</obo:IAO_0000115>
        <oboInOwl:hasOBONamespace>GAZ</oboInOwl:hasOBONamespace>
        <oboInOwl:id>GAZ:00031054</oboInOwl:id>
        <rdfs:label>Gogne District</rdfs:label>
    </owl:NamedIndividual>
    


    <!-- http://purl.obolibrary.org/obo/GAZ_00031055 -->

    <owl:NamedIndividual rdf:about="http://purl.obolibrary.org/obo/GAZ_00031055">
        <rdf:type rdf:resource="http://purl.obolibrary.org/obo/ENVO_00000856"/>
        <obo:RO_0001025 rdf:resource="http://purl.obolibrary.org/obo/GAZ_00230334"/>
        <obo:IAO_0000115>A populated place. A town in south-western Eritrea, lying south of Agordat.</obo:IAO_0000115>
        <oboInOwl:hasOBONamespace>GAZ</oboInOwl:hasOBONamespace>
        <oboInOwl:id>GAZ:00031055</oboInOwl:id>
        <rdfs:label>Barentu City</rdfs:label>
    </owl:NamedIndividual>
    


    <!-- http://purl.obolibrary.org/obo/GAZ_00031056 -->

    <owl:NamedIndividual rdf:about="http://purl.obolibrary.org/obo/GAZ_00031056">
        <rdf:type rdf:resource="http://purl.obolibrary.org/obo/ENVO_00000004"/>
        <obo:RO_0001025 rdf:resource="http://purl.obolibrary.org/obo/GAZ_00000774"/>
        <obo:IAO_0000115>A district in the Gash-Barka region of western Eritrea. The capital lies at Dghe.</obo:IAO_0000115>
        <oboInOwl:hasOBONamespace>GAZ</oboInOwl:hasOBONamespace>
        <oboInOwl:id>GAZ:00031056</oboInOwl:id>
        <rdfs:label>Dghe District</rdfs:label>
    </owl:NamedIndividual>
    


    <!-- http://purl.obolibrary.org/obo/GAZ_00031057 -->

    <owl:NamedIndividual rdf:about="http://purl.obolibrary.org/obo/GAZ_00031057">
        <rdf:type rdf:resource="http://purl.obolibrary.org/obo/ENVO_00000004"/>
        <obo:RO_0001025 rdf:resource="http://purl.obolibrary.org/obo/GAZ_00000774"/>
        <obo:IAO_0000115>A district in the Gash-Barka region of western Eritrea. The capital lies at Molki.</obo:IAO_0000115>
        <oboInOwl:hasOBONamespace>GAZ</oboInOwl:hasOBONamespace>
        <oboInOwl:id>GAZ:00031057</oboInOwl:id>
        <rdfs:label>Molki District</rdfs:label>
    </owl:NamedIndividual>
    


    <!-- http://purl.obolibrary.org/obo/GAZ_00031058 -->

    <owl:NamedIndividual rdf:about="http://purl.obolibrary.org/obo/GAZ_00031058">
        <rdf:type rdf:resource="http://purl.obolibrary.org/obo/ENVO_00000004"/>
        <obo:RO_0001025 rdf:resource="http://purl.obolibrary.org/obo/GAZ_00000774"/>
        <obo:IAO_0000115>A district in the Gash-Barka region of western Eritrea. The capital lies at Omhajer.</obo:IAO_0000115>
        <oboInOwl:hasOBONamespace>GAZ</oboInOwl:hasOBONamespace>
        <oboInOwl:id>GAZ:00031058</oboInOwl:id>
        <rdfs:label>Omhajer District</rdfs:label>
    </owl:NamedIndividual>
    


    <!-- http://purl.obolibrary.org/obo/GAZ_00031059 -->

    <owl:NamedIndividual rdf:about="http://purl.obolibrary.org/obo/GAZ_00031059">
        <rdf:type rdf:resource="http://purl.obolibrary.org/obo/ENVO_00000004"/>
        <obo:RO_0001025 rdf:resource="http://purl.obolibrary.org/obo/GAZ_00000774"/>
        <obo:IAO_0000115>A district in the Gash-Barka region of western Eritrea.</obo:IAO_0000115>
        <oboInOwl:hasOBONamespace>GAZ</oboInOwl:hasOBONamespace>
        <oboInOwl:id>GAZ:00031059</oboInOwl:id>
        <rdfs:label>Upper Gash District</rdfs:label>
    </owl:NamedIndividual>
    


    <!-- http://purl.obolibrary.org/obo/GAZ_00031060 -->

    <owl:NamedIndividual rdf:about="http://purl.obolibrary.org/obo/GAZ_00031060">
        <rdf:type rdf:resource="http://purl.obolibrary.org/obo/ENVO_00000004"/>
        <obo:RO_0001025 rdf:resource="http://purl.obolibrary.org/obo/GAZ_00000774"/>
        <obo:IAO_0000115>A district in the Gash-Barka region of western Eritrea. The capital lies at Teseney.</obo:IAO_0000115>
        <oboInOwl:hasOBONamespace>GAZ</oboInOwl:hasOBONamespace>
        <oboInOwl:id>GAZ:00031060</oboInOwl:id>
        <rdfs:label>Tesseney District</rdfs:label>
    </owl:NamedIndividual>
    


    <!-- http://purl.obolibrary.org/obo/GAZ_00031061 -->

    <owl:NamedIndividual rdf:about="http://purl.obolibrary.org/obo/GAZ_00031061">
        <rdf:type rdf:resource="http://purl.obolibrary.org/obo/ENVO_00000004"/>
        <obo:RO_0001025 rdf:resource="http://purl.obolibrary.org/obo/GAZ_00000774"/>
        <obo:IAO_0000115>A district in the Gash-Barka region of western Eritrea. The capital lies at Shambuko.</obo:IAO_0000115>
        <oboInOwl:hasOBONamespace>GAZ</oboInOwl:hasOBONamespace>
        <oboInOwl:id>GAZ:00031061</oboInOwl:id>
        <rdfs:label>Shambuko District</rdfs:label>
    </owl:NamedIndividual>
    


    <!-- http://purl.obolibrary.org/obo/GAZ_00031062 -->

    <owl:NamedIndividual rdf:about="http://purl.obolibrary.org/obo/GAZ_00031062">
        <rdf:type rdf:resource="http://purl.obolibrary.org/obo/ENVO_00000004"/>
        <obo:RO_0001025 rdf:resource="http://purl.obolibrary.org/obo/GAZ_00000774"/>
        <obo:IAO_0000115>A district in the Gash-Barka region of western Eritrea. The capital lies at Mogolo.</obo:IAO_0000115>
        <oboInOwl:hasOBONamespace>GAZ</oboInOwl:hasOBONamespace>
        <oboInOwl:id>GAZ:00031062</oboInOwl:id>
        <rdfs:label>Mogolo District</rdfs:label>
    </owl:NamedIndividual>
    


    <!-- http://purl.obolibrary.org/obo/GAZ_00031063 -->

    <owl:NamedIndividual rdf:about="http://purl.obolibrary.org/obo/GAZ_00031063">
        <obo:RO_0001025 rdf:resource="http://purl.obolibrary.org/obo/GAZ_00230331"/>
        <obo:IAO_0000115>A city. It lies in the west of Eritrea on the Barka River.</obo:IAO_0000115>
        <oboInOwl:hasOBONamespace>GAZ</oboInOwl:hasOBONamespace>
        <oboInOwl:id>GAZ:00031063</oboInOwl:id>
        <rdfs:label>Akurdet City</rdfs:label>
    </owl:NamedIndividual>
    


    <!-- http://purl.obolibrary.org/obo/GAZ_00031064 -->

    <owl:NamedIndividual rdf:about="http://purl.obolibrary.org/obo/GAZ_00031064">
        <rdf:type rdf:resource="http://purl.obolibrary.org/obo/ENVO_00000004"/>
        <obo:RO_0001025 rdf:resource="http://purl.obolibrary.org/obo/GAZ_10000775"/>
        <obo:IAO_0000115>A district in the Northern Red Sea region of Eritrea. The capital lies at Ghelalo.</obo:IAO_0000115>
        <oboInOwl:hasOBONamespace>GAZ</oboInOwl:hasOBONamespace>
        <oboInOwl:id>GAZ:00031064</oboInOwl:id>
        <rdfs:label>Ghelalo District</rdfs:label>
    </owl:NamedIndividual>
    


    <!-- http://purl.obolibrary.org/obo/GAZ_00031065 -->

    <owl:NamedIndividual rdf:about="http://purl.obolibrary.org/obo/GAZ_00031065">
        <rdf:type rdf:resource="http://purl.obolibrary.org/obo/ENVO_00000004"/>
        <obo:RO_0001025 rdf:resource="http://purl.obolibrary.org/obo/GAZ_10000775"/>
        <obo:IAO_0000115>A district in the Northern Red Sea region of Eritrea. The capital lies at Foro.</obo:IAO_0000115>
        <oboInOwl:hasOBONamespace>GAZ</oboInOwl:hasOBONamespace>
        <oboInOwl:id>GAZ:00031065</oboInOwl:id>
        <rdfs:label>Foro District</rdfs:label>
    </owl:NamedIndividual>
    


    <!-- http://purl.obolibrary.org/obo/GAZ_00031066 -->

    <owl:NamedIndividual rdf:about="http://purl.obolibrary.org/obo/GAZ_00031066">
        <rdf:type rdf:resource="http://purl.obolibrary.org/obo/ENVO_00000004"/>
        <obo:RO_0001025 rdf:resource="http://purl.obolibrary.org/obo/GAZ_10000775"/>
        <obo:IAO_0000115>A district in the Northern Red Sea region of Eritrea. The capital lies at Afabet.</obo:IAO_0000115>
        <oboInOwl:hasOBONamespace>GAZ</oboInOwl:hasOBONamespace>
        <oboInOwl:id>GAZ:00031066</oboInOwl:id>
        <rdfs:label>Af&apos;abet District</rdfs:label>
    </owl:NamedIndividual>
    


    <!-- http://purl.obolibrary.org/obo/GAZ_00031067 -->

    <owl:NamedIndividual rdf:about="http://purl.obolibrary.org/obo/GAZ_00031067">
        <rdf:type rdf:resource="http://purl.obolibrary.org/obo/ENVO_00000004"/>
        <obo:RO_0001025 rdf:resource="http://purl.obolibrary.org/obo/GAZ_10000775"/>
        <obo:IAO_0000115>A district in the Northern Red Sea region of Eritrea. The capital lies at Massawa.</obo:IAO_0000115>
        <oboInOwl:hasOBONamespace>GAZ</oboInOwl:hasOBONamespace>
        <oboInOwl:id>GAZ:00031067</oboInOwl:id>
        <rdfs:label>Massawa District</rdfs:label>
    </owl:NamedIndividual>
    


    <!-- http://purl.obolibrary.org/obo/GAZ_00031068 -->

    <owl:NamedIndividual rdf:about="http://purl.obolibrary.org/obo/GAZ_00031068">
        <rdf:type rdf:resource="http://purl.obolibrary.org/obo/ENVO_00000004"/>
        <obo:RO_0001025 rdf:resource="http://purl.obolibrary.org/obo/GAZ_10000775"/>
        <obo:IAO_0000115>A district in the Northern Red Sea region of Eritrea. It is the administrative sub-region that covers the islands of the Dahlak Archipelago.</obo:IAO_0000115>
        <oboInOwl:hasOBONamespace>GAZ</oboInOwl:hasOBONamespace>
        <oboInOwl:id>GAZ:00031068</oboInOwl:id>
        <rdfs:label>Dahlak District</rdfs:label>
    </owl:NamedIndividual>
    


    <!-- http://purl.obolibrary.org/obo/GAZ_00031069 -->

    <owl:NamedIndividual rdf:about="http://purl.obolibrary.org/obo/GAZ_00031069">
        <rdf:type rdf:resource="http://purl.obolibrary.org/obo/ENVO_00000004"/>
        <obo:RO_0001025 rdf:resource="http://purl.obolibrary.org/obo/GAZ_10000775"/>
        <obo:IAO_0000115>A district in the Northern Red Sea region of Eritrea. The capital lies at Ghinda.</obo:IAO_0000115>
        <oboInOwl:hasOBONamespace>GAZ</oboInOwl:hasOBONamespace>
        <oboInOwl:id>GAZ:00031069</oboInOwl:id>
        <rdfs:label>Ghinda District</rdfs:label>
    </owl:NamedIndividual>
    


    <!-- http://purl.obolibrary.org/obo/GAZ_00031070 -->

    <owl:NamedIndividual rdf:about="http://purl.obolibrary.org/obo/GAZ_00031070">
        <rdf:type rdf:resource="http://purl.obolibrary.org/obo/ENVO_00000004"/>
        <obo:RO_0001025 rdf:resource="http://purl.obolibrary.org/obo/GAZ_10000775"/>
        <obo:IAO_0000115>A district in the Northern Red Sea region of Eritrea. The district capital is Karura.</obo:IAO_0000115>
        <oboInOwl:hasOBONamespace>GAZ</oboInOwl:hasOBONamespace>
        <oboInOwl:id>GAZ:00031070</oboInOwl:id>
        <rdfs:label>Karura District</rdfs:label>
    </owl:NamedIndividual>
    


    <!-- http://purl.obolibrary.org/obo/GAZ_00031071 -->

    <owl:NamedIndividual rdf:about="http://purl.obolibrary.org/obo/GAZ_00031071">
        <rdf:type rdf:resource="http://purl.obolibrary.org/obo/ENVO_00000004"/>
        <obo:RO_0001025 rdf:resource="http://purl.obolibrary.org/obo/GAZ_10000775"/>
        <obo:IAO_0000115>A district in the Northern Red Sea region of Eritrea. The capital lies at Nakfa.</obo:IAO_0000115>
        <oboInOwl:hasOBONamespace>GAZ</oboInOwl:hasOBONamespace>
        <oboInOwl:id>GAZ:00031071</oboInOwl:id>
        <rdfs:label>Nakfa District</rdfs:label>
    </owl:NamedIndividual>
    


    <!-- http://purl.obolibrary.org/obo/GAZ_00031072 -->

    <owl:NamedIndividual rdf:about="http://purl.obolibrary.org/obo/GAZ_00031072">
        <rdf:type rdf:resource="http://purl.obolibrary.org/obo/ENVO_00000004"/>
        <obo:RO_0001025 rdf:resource="http://purl.obolibrary.org/obo/GAZ_10000775"/>
        <obo:IAO_0000115>A district in the Northern Red Sea region of Eritrea. The capital lies at She&apos;eb.</obo:IAO_0000115>
        <oboInOwl:hasOBONamespace>GAZ</oboInOwl:hasOBONamespace>
        <oboInOwl:id>GAZ:00031072</oboInOwl:id>
        <rdfs:label>She&apos;eb District</rdfs:label>
    </owl:NamedIndividual>
    


    <!-- http://purl.obolibrary.org/obo/GAZ_00031073 -->

    <owl:NamedIndividual rdf:about="http://purl.obolibrary.org/obo/GAZ_00031073">
        <rdf:type rdf:resource="http://purl.obolibrary.org/obo/ENVO_00000004"/>
        <obo:RO_0001025 rdf:resource="http://purl.obolibrary.org/obo/GAZ_00000776"/>
        <obo:IAO_0000115>A district in the Debub region of Eritrea. The capital lies at Kudo Be&apos;ur.</obo:IAO_0000115>
        <oboInOwl:hasOBONamespace>GAZ</oboInOwl:hasOBONamespace>
        <oboInOwl:id>GAZ:00031073</oboInOwl:id>
        <rdfs:label>Kudo Be&apos;ur District</rdfs:label>
    </owl:NamedIndividual>
    


    <!-- http://purl.obolibrary.org/obo/GAZ_00031074 -->

    <owl:NamedIndividual rdf:about="http://purl.obolibrary.org/obo/GAZ_00031074">
        <rdf:type rdf:resource="http://purl.obolibrary.org/obo/ENVO_00000004"/>
        <obo:RO_0001025 rdf:resource="http://purl.obolibrary.org/obo/GAZ_00000776"/>
        <obo:IAO_0000115>A district in the Debub region of Eritrea. The capital lies at Areza.</obo:IAO_0000115>
        <oboInOwl:hasOBONamespace>GAZ</oboInOwl:hasOBONamespace>
        <oboInOwl:id>GAZ:00031074</oboInOwl:id>
        <rdfs:label>Areza District</rdfs:label>
    </owl:NamedIndividual>
    


    <!-- http://purl.obolibrary.org/obo/GAZ_00031075 -->

    <owl:NamedIndividual rdf:about="http://purl.obolibrary.org/obo/GAZ_00031075">
        <rdf:type rdf:resource="http://purl.obolibrary.org/obo/ENVO_00000004"/>
        <obo:RO_0001025 rdf:resource="http://purl.obolibrary.org/obo/GAZ_00000777"/>
        <obo:IAO_0000115>A district in the Southern Red Sea region of southern Eritrea.</obo:IAO_0000115>
        <oboInOwl:hasOBONamespace>GAZ</oboInOwl:hasOBONamespace>
        <oboInOwl:id>GAZ:00031075</oboInOwl:id>
        <rdfs:label>Central Denkalya District</rdfs:label>
    </owl:NamedIndividual>
    


    <!-- http://purl.obolibrary.org/obo/GAZ_00031076 -->

    <owl:NamedIndividual rdf:about="http://purl.obolibrary.org/obo/GAZ_00031076">
        <rdf:type rdf:resource="http://purl.obolibrary.org/obo/ENVO_00000004"/>
        <obo:RO_0001025 rdf:resource="http://purl.obolibrary.org/obo/GAZ_00000776"/>
        <obo:IAO_0000115>A district in the Debub region of Eritrea. The capital lies at Adi Keyh.</obo:IAO_0000115>
        <oboInOwl:hasOBONamespace>GAZ</oboInOwl:hasOBONamespace>
        <oboInOwl:id>GAZ:00031076</oboInOwl:id>
        <rdfs:label>Adi Keyh District</rdfs:label>
    </owl:NamedIndividual>
    


    <!-- http://purl.obolibrary.org/obo/GAZ_00031077 -->

    <owl:NamedIndividual rdf:about="http://purl.obolibrary.org/obo/GAZ_00031077">
        <rdf:type rdf:resource="http://purl.obolibrary.org/obo/ENVO_00000004"/>
        <obo:RO_0001025 rdf:resource="http://purl.obolibrary.org/obo/GAZ_00000777"/>
        <obo:IAO_0000115>A district in the Southern Red Sea region of southern Eritrea.</obo:IAO_0000115>
        <oboInOwl:hasOBONamespace>GAZ</oboInOwl:hasOBONamespace>
        <oboInOwl:id>GAZ:00031077</oboInOwl:id>
        <rdfs:label>Southern Denkalya District</rdfs:label>
    </owl:NamedIndividual>
    


    <!-- http://purl.obolibrary.org/obo/GAZ_00031078 -->

    <owl:NamedIndividual rdf:about="http://purl.obolibrary.org/obo/GAZ_00031078">
        <rdf:type rdf:resource="http://purl.obolibrary.org/obo/ENVO_00000004"/>
        <obo:RO_0001025 rdf:resource="http://purl.obolibrary.org/obo/GAZ_00000776"/>
        <obo:IAO_0000115>A district in the Debub region of Eritrea. The capital lies at Dekemhare.</obo:IAO_0000115>
        <oboInOwl:hasOBONamespace>GAZ</oboInOwl:hasOBONamespace>
        <oboInOwl:id>GAZ:00031078</oboInOwl:id>
        <rdfs:label>Dekemhare District</rdfs:label>
    </owl:NamedIndividual>
    


    <!-- http://purl.obolibrary.org/obo/GAZ_00031079 -->

    <owl:NamedIndividual rdf:about="http://purl.obolibrary.org/obo/GAZ_00031079">
        <rdf:type rdf:resource="http://purl.obolibrary.org/obo/ENVO_00000004"/>
        <obo:RO_0001025 rdf:resource="http://purl.obolibrary.org/obo/GAZ_00000777"/>
        <obo:IAO_0000115>A district in the Southern Red Sea region of southern Eritrea. The capital lies at Tiyo.</obo:IAO_0000115>
        <oboInOwl:hasOBONamespace>GAZ</oboInOwl:hasOBONamespace>
        <oboInOwl:id>GAZ:00031079</oboInOwl:id>
        <rdfs:label>Are&apos;eta District</rdfs:label>
    </owl:NamedIndividual>
    


    <!-- http://purl.obolibrary.org/obo/GAZ_00031080 -->

    <owl:NamedIndividual rdf:about="http://purl.obolibrary.org/obo/GAZ_00031080">
        <rdf:type rdf:resource="http://purl.obolibrary.org/obo/ENVO_00000004"/>
        <obo:RO_0001025 rdf:resource="http://purl.obolibrary.org/obo/GAZ_00000776"/>
        <obo:IAO_0000115>A district in the Debub region of Eritrea. The capital lies at Mendefera.</obo:IAO_0000115>
        <oboInOwl:hasOBONamespace>GAZ</oboInOwl:hasOBONamespace>
        <oboInOwl:id>GAZ:00031080</oboInOwl:id>
        <rdfs:label>Mendefera District</rdfs:label>
    </owl:NamedIndividual>
    


    <!-- http://purl.obolibrary.org/obo/GAZ_00031081 -->

    <owl:NamedIndividual rdf:about="http://purl.obolibrary.org/obo/GAZ_00031081">
        <rdf:type rdf:resource="http://purl.obolibrary.org/obo/ENVO_00000004"/>
        <obo:RO_0001025 rdf:resource="http://purl.obolibrary.org/obo/GAZ_00000776"/>
        <obo:IAO_0000115>A district in the Debub region of Eritrea. The capital lies at Debarwa.</obo:IAO_0000115>
        <oboInOwl:hasOBONamespace>GAZ</oboInOwl:hasOBONamespace>
        <oboInOwl:id>GAZ:00031081</oboInOwl:id>
        <rdfs:label>Debarwa District</rdfs:label>
    </owl:NamedIndividual>
    


    <!-- http://purl.obolibrary.org/obo/GAZ_00031082 -->

    <owl:NamedIndividual rdf:about="http://purl.obolibrary.org/obo/GAZ_00031082">
        <rdf:type rdf:resource="http://purl.obolibrary.org/obo/ENVO_00000004"/>
        <obo:RO_0001025 rdf:resource="http://purl.obolibrary.org/obo/GAZ_00000776"/>
        <obo:IAO_0000115>A district in the Debub region of Eritrea. The capital lies at Adi Quala.</obo:IAO_0000115>
        <oboInOwl:hasOBONamespace>GAZ</oboInOwl:hasOBONamespace>
        <oboInOwl:id>GAZ:00031082</oboInOwl:id>
        <rdfs:label>Adi Quala District</rdfs:label>
    </owl:NamedIndividual>
    


    <!-- http://purl.obolibrary.org/obo/GAZ_00031083 -->

    <owl:NamedIndividual rdf:about="http://purl.obolibrary.org/obo/GAZ_00031083">
        <rdf:type rdf:resource="http://purl.obolibrary.org/obo/ENVO_00000004"/>
        <obo:RO_0001025 rdf:resource="http://purl.obolibrary.org/obo/GAZ_00000776"/>
        <obo:IAO_0000115>A district in the Debub region of Eritrea. The capital lies at Segeneiti.</obo:IAO_0000115>
        <oboInOwl:hasOBONamespace>GAZ</oboInOwl:hasOBONamespace>
        <oboInOwl:id>GAZ:00031083</oboInOwl:id>
        <rdfs:label>Segeneiti District</rdfs:label>
    </owl:NamedIndividual>
    


    <!-- http://purl.obolibrary.org/obo/GAZ_00031084 -->

    <owl:NamedIndividual rdf:about="http://purl.obolibrary.org/obo/GAZ_00031084">
        <rdf:type rdf:resource="http://purl.obolibrary.org/obo/ENVO_00000004"/>
        <obo:RO_0001025 rdf:resource="http://purl.obolibrary.org/obo/GAZ_00000776"/>
        <obo:IAO_0000115>A district in the Debub region of Eritrea. The capital lies at Mai-Mne.</obo:IAO_0000115>
        <oboInOwl:hasOBONamespace>GAZ</oboInOwl:hasOBONamespace>
        <oboInOwl:id>GAZ:00031084</oboInOwl:id>
        <rdfs:label>Mai-Mne District</rdfs:label>
    </owl:NamedIndividual>
    


    <!-- http://purl.obolibrary.org/obo/GAZ_00031085 -->

    <owl:NamedIndividual rdf:about="http://purl.obolibrary.org/obo/GAZ_00031085">
        <rdf:type rdf:resource="http://purl.obolibrary.org/obo/ENVO_00000004"/>
        <obo:RO_0001025 rdf:resource="http://purl.obolibrary.org/obo/GAZ_00000776"/>
        <obo:IAO_0000115>A district in the Debub region of Eritrea. The capital lies at Senafe.</obo:IAO_0000115>
        <oboInOwl:hasOBONamespace>GAZ</oboInOwl:hasOBONamespace>
        <oboInOwl:id>GAZ:00031085</oboInOwl:id>
        <rdfs:label>Senafe District</rdfs:label>
    </owl:NamedIndividual>
    


    <!-- http://purl.obolibrary.org/obo/GAZ_00039909 -->

    <owl:NamedIndividual rdf:about="http://purl.obolibrary.org/obo/GAZ_00039909">
        <obo:RO_0001025 rdf:resource="http://purl.obolibrary.org/obo/GAZ_00009683"/>
        <obo:IAO_0000115>An island of the Dahlak Archipelago.</obo:IAO_0000115>
        <oboInOwl:hasOBONamespace>GAZ</oboInOwl:hasOBONamespace>
        <oboInOwl:id>GAZ:00039909</oboInOwl:id>
        <rdfs:label>Harmil Island</rdfs:label>
    </owl:NamedIndividual>
    


    <!-- http://purl.obolibrary.org/obo/GAZ_00039910 -->

    <owl:NamedIndividual rdf:about="http://purl.obolibrary.org/obo/GAZ_00039910">
        <obo:RO_0001025 rdf:resource="http://purl.obolibrary.org/obo/GAZ_00009683"/>
        <obo:IAO_0000115>An island of the Dahlak Archipelago.</obo:IAO_0000115>
        <oboInOwl:hasOBONamespace>GAZ</oboInOwl:hasOBONamespace>
        <oboInOwl:id>GAZ:00039910</oboInOwl:id>
        <rdfs:label>Nora Island</rdfs:label>
    </owl:NamedIndividual>
    


    <!-- http://purl.obolibrary.org/obo/GAZ_00039911 -->

    <owl:NamedIndividual rdf:about="http://purl.obolibrary.org/obo/GAZ_00039911">
        <obo:RO_0001025 rdf:resource="http://purl.obolibrary.org/obo/GAZ_00009683"/>
        <obo:IAO_0000115>An island of the Dahlak Archipelago.</obo:IAO_0000115>
        <oboInOwl:hasOBONamespace>GAZ</oboInOwl:hasOBONamespace>
        <oboInOwl:id>GAZ:00039911</oboInOwl:id>
        <rdfs:label>Dahlak Kebir</rdfs:label>
    </owl:NamedIndividual>
    


    <!-- http://purl.obolibrary.org/obo/GAZ_00039912 -->

    <owl:NamedIndividual rdf:about="http://purl.obolibrary.org/obo/GAZ_00039912">
        <obo:RO_0001025 rdf:resource="http://purl.obolibrary.org/obo/GAZ_00009683"/>
        <obo:IAO_0000115>An island of the Dahlak Archipelago.</obo:IAO_0000115>
        <oboInOwl:hasOBONamespace>GAZ</oboInOwl:hasOBONamespace>
        <oboInOwl:id>GAZ:00039912</oboInOwl:id>
        <rdfs:label>Nahaleg Island</rdfs:label>
    </owl:NamedIndividual>
    


    <!-- http://purl.obolibrary.org/obo/GAZ_00039913 -->

    <owl:NamedIndividual rdf:about="http://purl.obolibrary.org/obo/GAZ_00039913">
        <obo:RO_0001025 rdf:resource="http://purl.obolibrary.org/obo/GAZ_00031067"/>
        <obo:IAO_0000115>An island.</obo:IAO_0000115>
        <oboInOwl:hasOBONamespace>GAZ</oboInOwl:hasOBONamespace>
        <oboInOwl:id>GAZ:00039913</oboInOwl:id>
        <rdfs:label>Massawa Island</rdfs:label>
    </owl:NamedIndividual>
    


    <!-- http://purl.obolibrary.org/obo/GAZ_00039915 -->

    <owl:NamedIndividual rdf:about="http://purl.obolibrary.org/obo/GAZ_00039915">
        <obo:RO_0001025 rdf:resource="http://purl.obolibrary.org/obo/GAZ_00248117"/>
        <obo:IAO_0000115>An island.</obo:IAO_0000115>
        <oboInOwl:hasOBONamespace>GAZ</oboInOwl:hasOBONamespace>
        <oboInOwl:id>GAZ:00039915</oboInOwl:id>
        <rdfs:label>Halba Deset</rdfs:label>
    </owl:NamedIndividual>
    


    <!-- http://purl.obolibrary.org/obo/GAZ_00039916 -->

    <owl:NamedIndividual rdf:about="http://purl.obolibrary.org/obo/GAZ_00039916">
        <obo:RO_0001025 rdf:resource="http://purl.obolibrary.org/obo/GAZ_10000775"/>
        <obo:IAO_0000115>Islands.</obo:IAO_0000115>
        <oboInOwl:hasOBONamespace>GAZ</oboInOwl:hasOBONamespace>
        <oboInOwl:id>GAZ:00039916</oboInOwl:id>
        <rdfs:label>Howakil Islands</rdfs:label>
    </owl:NamedIndividual>
    


    <!-- http://purl.obolibrary.org/obo/GAZ_00039917 -->

    <owl:NamedIndividual rdf:about="http://purl.obolibrary.org/obo/GAZ_00039917">
        <obo:RO_0001025 rdf:resource="http://purl.obolibrary.org/obo/GAZ_00009683"/>
        <obo:IAO_0000115>An island of the Dahlak Archipelago.</obo:IAO_0000115>
        <oboInOwl:hasOBONamespace>GAZ</oboInOwl:hasOBONamespace>
        <oboInOwl:id>GAZ:00039917</oboInOwl:id>
        <rdfs:label>Isra-Tu Island</rdfs:label>
    </owl:NamedIndividual>
    


    <!-- http://purl.obolibrary.org/obo/GAZ_00039918 -->

    <owl:NamedIndividual rdf:about="http://purl.obolibrary.org/obo/GAZ_00039918">
        <obo:RO_0001025 rdf:resource="http://purl.obolibrary.org/obo/GAZ_00009683"/>
        <obo:IAO_0000115>An island of the Dahlak Archipelago.</obo:IAO_0000115>
        <oboInOwl:hasOBONamespace>GAZ</oboInOwl:hasOBONamespace>
        <oboInOwl:id>GAZ:00039918</oboInOwl:id>
        <rdfs:label>Shumma Island</rdfs:label>
    </owl:NamedIndividual>
    


    <!-- http://purl.obolibrary.org/obo/GAZ_00039919 -->

    <owl:NamedIndividual rdf:about="http://purl.obolibrary.org/obo/GAZ_00039919">
        <obo:RO_0001025 rdf:resource="http://purl.obolibrary.org/obo/GAZ_00009683"/>
        <obo:IAO_0000115>An island of the Dahlak Archipelago.</obo:IAO_0000115>
        <oboInOwl:hasOBONamespace>GAZ</oboInOwl:hasOBONamespace>
        <oboInOwl:id>GAZ:00039919</oboInOwl:id>
        <rdfs:label>Harat Island</rdfs:label>
    </owl:NamedIndividual>
    


    <!-- http://purl.obolibrary.org/obo/GAZ_00039920 -->

    <owl:NamedIndividual rdf:about="http://purl.obolibrary.org/obo/GAZ_00039920">
        <obo:RO_0001025 rdf:resource="http://purl.obolibrary.org/obo/GAZ_00009683"/>
        <obo:IAO_0000115>An island of the Dahlak Archipelago.</obo:IAO_0000115>
        <oboInOwl:hasOBONamespace>GAZ</oboInOwl:hasOBONamespace>
        <oboInOwl:id>GAZ:00039920</oboInOwl:id>
        <rdfs:label>Dissei Island</rdfs:label>
    </owl:NamedIndividual>
    


    <!-- http://purl.obolibrary.org/obo/GAZ_00039921 -->

    <owl:NamedIndividual rdf:about="http://purl.obolibrary.org/obo/GAZ_00039921">
        <obo:RO_0001025 rdf:resource="http://purl.obolibrary.org/obo/GAZ_00009683"/>
        <obo:IAO_0000115>An island of the Dahlak Archipelago.</obo:IAO_0000115>
        <oboInOwl:hasOBONamespace>GAZ</oboInOwl:hasOBONamespace>
        <oboInOwl:id>GAZ:00039921</oboInOwl:id>
        <rdfs:label>Erwa Island</rdfs:label>
    </owl:NamedIndividual>
    


    <!-- http://purl.obolibrary.org/obo/GAZ_00039922 -->

    <owl:NamedIndividual rdf:about="http://purl.obolibrary.org/obo/GAZ_00039922">
        <obo:RO_0001025 rdf:resource="http://purl.obolibrary.org/obo/GAZ_00009683"/>
        <obo:IAO_0000115>An island of the Dahlak Archipelago.</obo:IAO_0000115>
        <oboInOwl:hasOBONamespace>GAZ</oboInOwl:hasOBONamespace>
        <oboInOwl:id>GAZ:00039922</oboInOwl:id>
        <rdfs:label>Dohul Island</rdfs:label>
    </owl:NamedIndividual>
    


    <!-- http://purl.obolibrary.org/obo/GAZ_00039923 -->

    <owl:NamedIndividual rdf:about="http://purl.obolibrary.org/obo/GAZ_00039923">
        <obo:RO_0001025 rdf:resource="http://purl.obolibrary.org/obo/GAZ_00009683"/>
        <obo:IAO_0000115>An island of the Dahlak Archipelago.</obo:IAO_0000115>
        <oboInOwl:hasOBONamespace>GAZ</oboInOwl:hasOBONamespace>
        <oboInOwl:id>GAZ:00039923</oboInOwl:id>
        <rdfs:label>Dhuladhiya Island</rdfs:label>
    </owl:NamedIndividual>
    


    <!-- http://purl.obolibrary.org/obo/GAZ_00040045 -->

    <owl:NamedIndividual rdf:about="http://purl.obolibrary.org/obo/GAZ_00040045">
        <obo:RO_0001025 rdf:resource="http://purl.obolibrary.org/obo/GAZ_00015452"/>
        <obo:IAO_0000115>An archipelago of eighty-four islands in the northwest of Lake Victoria, Uganda. The islands lie in two main groups, separated by the Kkome Channel.</obo:IAO_0000115>
        <oboInOwl:hasOBONamespace>GAZ</oboInOwl:hasOBONamespace>
        <oboInOwl:id>GAZ:00040045</oboInOwl:id>
        <rdfs:label>Ssese Islands</rdfs:label>
    </owl:NamedIndividual>
    


    <!-- http://purl.obolibrary.org/obo/GAZ_00040046 -->

    <owl:NamedIndividual rdf:about="http://purl.obolibrary.org/obo/GAZ_00040046">
        <obo:RO_0001025 rdf:resource="http://purl.obolibrary.org/obo/GAZ_00040045"/>
        <oboInOwl:hasOBONamespace>GAZ</oboInOwl:hasOBONamespace>
        <oboInOwl:id>GAZ:00040046</oboInOwl:id>
        <rdfs:label>Northeast Ssese Islands</rdfs:label>
    </owl:NamedIndividual>
    


    <!-- http://purl.obolibrary.org/obo/GAZ_00040047 -->

    <owl:NamedIndividual rdf:about="http://purl.obolibrary.org/obo/GAZ_00040047">
        <obo:RO_0001025 rdf:resource="http://purl.obolibrary.org/obo/GAZ_00040045"/>
        <oboInOwl:hasOBONamespace>GAZ</oboInOwl:hasOBONamespace>
        <oboInOwl:id>GAZ:00040047</oboInOwl:id>
        <rdfs:label>Southwest Ssese Islands</rdfs:label>
    </owl:NamedIndividual>
    


    <!-- http://purl.obolibrary.org/obo/GAZ_00040048 -->

    <owl:NamedIndividual rdf:about="http://purl.obolibrary.org/obo/GAZ_00040048">
        <obo:RO_0001025 rdf:resource="http://purl.obolibrary.org/obo/GAZ_00040046"/>
        <oboInOwl:hasOBONamespace>GAZ</oboInOwl:hasOBONamespace>
        <oboInOwl:id>GAZ:00040048</oboInOwl:id>
        <rdfs:label>Damba Island</rdfs:label>
    </owl:NamedIndividual>
    


    <!-- http://purl.obolibrary.org/obo/GAZ_00040049 -->

    <owl:NamedIndividual rdf:about="http://purl.obolibrary.org/obo/GAZ_00040049">
        <obo:RO_0001025 rdf:resource="http://purl.obolibrary.org/obo/GAZ_00040046"/>
        <oboInOwl:hasOBONamespace>GAZ</oboInOwl:hasOBONamespace>
        <oboInOwl:id>GAZ:00040049</oboInOwl:id>
        <rdfs:label>Kkome Island</rdfs:label>
    </owl:NamedIndividual>
    


    <!-- http://purl.obolibrary.org/obo/GAZ_00040050 -->

    <owl:NamedIndividual rdf:about="http://purl.obolibrary.org/obo/GAZ_00040050">
        <obo:RO_0001025 rdf:resource="http://purl.obolibrary.org/obo/GAZ_00040046"/>
        <oboInOwl:hasOBONamespace>GAZ</oboInOwl:hasOBONamespace>
        <oboInOwl:id>GAZ:00040050</oboInOwl:id>
        <rdfs:label>Luwaji Island</rdfs:label>
    </owl:NamedIndividual>
    


    <!-- http://purl.obolibrary.org/obo/GAZ_00040051 -->

    <owl:NamedIndividual rdf:about="http://purl.obolibrary.org/obo/GAZ_00040051">
        <obo:RO_0001025 rdf:resource="http://purl.obolibrary.org/obo/GAZ_00040047"/>
        <oboInOwl:hasOBONamespace>GAZ</oboInOwl:hasOBONamespace>
        <oboInOwl:id>GAZ:00040051</oboInOwl:id>
        <rdfs:label>Buyova Island</rdfs:label>
    </owl:NamedIndividual>
    


    <!-- http://purl.obolibrary.org/obo/GAZ_00040052 -->

    <owl:NamedIndividual rdf:about="http://purl.obolibrary.org/obo/GAZ_00040052">
        <obo:RO_0001025 rdf:resource="http://purl.obolibrary.org/obo/GAZ_00040047"/>
        <oboInOwl:hasOBONamespace>GAZ</oboInOwl:hasOBONamespace>
        <oboInOwl:id>GAZ:00040052</oboInOwl:id>
        <rdfs:label>Serinya Island</rdfs:label>
    </owl:NamedIndividual>
    


    <!-- http://purl.obolibrary.org/obo/GAZ_00040053 -->

    <owl:NamedIndividual rdf:about="http://purl.obolibrary.org/obo/GAZ_00040053">
        <obo:RO_0001025 rdf:resource="http://purl.obolibrary.org/obo/GAZ_00040047"/>
        <oboInOwl:hasOBONamespace>GAZ</oboInOwl:hasOBONamespace>
        <oboInOwl:id>GAZ:00040053</oboInOwl:id>
        <rdfs:label>Funve Island</rdfs:label>
    </owl:NamedIndividual>
    


    <!-- http://purl.obolibrary.org/obo/GAZ_00040054 -->

    <owl:NamedIndividual rdf:about="http://purl.obolibrary.org/obo/GAZ_00040054">
        <obo:RO_0001025 rdf:resource="http://purl.obolibrary.org/obo/GAZ_00040047"/>
        <obo:IAO_0000115>The second largest island in Lake Victoria, Uganda, after Ukerewe. Its area is 275 km2. It is a part of the Ssese Islands in the Kalangala District. Chief town is Kalangala.</obo:IAO_0000115>
        <oboInOwl:hasOBONamespace>GAZ</oboInOwl:hasOBONamespace>
        <oboInOwl:id>GAZ:00040054</oboInOwl:id>
        <rdfs:label>Bugala Island</rdfs:label>
    </owl:NamedIndividual>
    


    <!-- http://purl.obolibrary.org/obo/GAZ_00040055 -->

    <owl:NamedIndividual rdf:about="http://purl.obolibrary.org/obo/GAZ_00040055">
        <obo:RO_0001025 rdf:resource="http://purl.obolibrary.org/obo/GAZ_00040047"/>
        <oboInOwl:hasOBONamespace>GAZ</oboInOwl:hasOBONamespace>
        <oboInOwl:id>GAZ:00040055</oboInOwl:id>
        <rdfs:label>Bufumira Island</rdfs:label>
    </owl:NamedIndividual>
    


    <!-- http://purl.obolibrary.org/obo/GAZ_00040056 -->

    <owl:NamedIndividual rdf:about="http://purl.obolibrary.org/obo/GAZ_00040056">
        <obo:RO_0001025 rdf:resource="http://purl.obolibrary.org/obo/GAZ_00040047"/>
        <oboInOwl:hasOBONamespace>GAZ</oboInOwl:hasOBONamespace>
        <oboInOwl:id>GAZ:00040056</oboInOwl:id>
        <rdfs:label>Bukasa Island</rdfs:label>
    </owl:NamedIndividual>
    


    <!-- http://purl.obolibrary.org/obo/GAZ_00040057 -->

    <owl:NamedIndividual rdf:about="http://purl.obolibrary.org/obo/GAZ_00040057">
        <obo:RO_0001025 rdf:resource="http://purl.obolibrary.org/obo/GAZ_00040047"/>
        <oboInOwl:hasOBONamespace>GAZ</oboInOwl:hasOBONamespace>
        <oboInOwl:id>GAZ:00040057</oboInOwl:id>
        <rdfs:label>Bugaba Island</rdfs:label>
    </owl:NamedIndividual>
    


    <!-- http://purl.obolibrary.org/obo/GAZ_00040058 -->

    <owl:NamedIndividual rdf:about="http://purl.obolibrary.org/obo/GAZ_00040058">
        <obo:RO_0001025 rdf:resource="http://purl.obolibrary.org/obo/GAZ_00040047"/>
        <oboInOwl:hasOBONamespace>GAZ</oboInOwl:hasOBONamespace>
        <oboInOwl:id>GAZ:00040058</oboInOwl:id>
        <rdfs:label>Bubeke Island</rdfs:label>
    </owl:NamedIndividual>
    


    <!-- http://purl.obolibrary.org/obo/GAZ_00041527 -->

    <owl:NamedIndividual rdf:about="http://purl.obolibrary.org/obo/GAZ_00041527">
        <obo:RO_0001025 rdf:resource="http://purl.obolibrary.org/obo/GAZ_00015452"/>
        <obo:IAO_0000115>The largest island in Lake Victoria, the largest inland island in Africa. Located 45 km north of Mwanza.</obo:IAO_0000115>
        <oboInOwl:hasOBONamespace>GAZ</oboInOwl:hasOBONamespace>
        <oboInOwl:id>GAZ:00041527</oboInOwl:id>
        <rdfs:label>Ukerewe Island</rdfs:label>
    </owl:NamedIndividual>
    


    <!-- http://purl.obolibrary.org/obo/GAZ_00041528 -->

    <owl:NamedIndividual rdf:about="http://purl.obolibrary.org/obo/GAZ_00041528">
        <obo:RO_0001025 rdf:resource="http://purl.obolibrary.org/obo/GAZ_00000007"/>
        <obo:IAO_0000115>An endorheic lake, in western Zomba District of Malawi, near the border with Mozambique.</obo:IAO_0000115>
        <oboInOwl:hasOBONamespace>GAZ</oboInOwl:hasOBONamespace>
        <oboInOwl:id>GAZ:00041528</oboInOwl:id>
        <rdfs:label>Lake Chilwa</rdfs:label>
    </owl:NamedIndividual>
    


    <!-- http://purl.obolibrary.org/obo/GAZ_00041529 -->

    <owl:NamedIndividual rdf:about="http://purl.obolibrary.org/obo/GAZ_00041529">
        <obo:RO_0001025 rdf:resource="http://purl.obolibrary.org/obo/GAZ_00000007"/>
        <obo:IAO_0000115>A lake in southern part of Malawi, in the Southern Region.</obo:IAO_0000115>
        <oboInOwl:hasOBONamespace>GAZ</oboInOwl:hasOBONamespace>
        <oboInOwl:id>GAZ:00041529</oboInOwl:id>
        <rdfs:label>Lake Malombe</rdfs:label>
    </owl:NamedIndividual>
    


    <!-- http://purl.obolibrary.org/obo/GAZ_00041530 -->

    <owl:NamedIndividual rdf:about="http://purl.obolibrary.org/obo/GAZ_00041530">
        <obo:RO_0001025 rdf:resource="http://purl.obolibrary.org/obo/GAZ_00000007"/>
        <obo:IAO_0000115>A freshwater lake on the longest arm of Africa&apos;s second-longest river, the Congo. Located on the border between Zambia and Democratic Republic of the Congo, it makes up 110 km of the total length of the Congo, lying between its Luapula River (upstream) and Luvua River (downstream) segments. Mweru is mainly fed by the Luapula River, which comes in through swamps from the south, and the Kalungwishi River from the east. At its north end the lake is drained by the Luvua River, which flows in a northwesterly direction to join the Lualaba River and thence to the Congo.</obo:IAO_0000115>
        <oboInOwl:hasOBONamespace>GAZ</oboInOwl:hasOBONamespace>
        <oboInOwl:id>GAZ:00041530</oboInOwl:id>
        <rdfs:label>Lake Mweru</rdfs:label>
    </owl:NamedIndividual>
    


    <!-- http://purl.obolibrary.org/obo/GAZ_00041531 -->

    <owl:NamedIndividual rdf:about="http://purl.obolibrary.org/obo/GAZ_00041531">
        <obo:RO_0001025 rdf:resource="http://purl.obolibrary.org/obo/GAZ_00000007"/>
        <obo:IAO_0000115>An alkaline lake in southwestern Tanzania. It is divided into two basins by a central swamp zone, ranging from 5-20 km wide. It is fed by 17 rivers. Seven rivers enter the south basin and 10 discharge to the north basin.</obo:IAO_0000115>
        <oboInOwl:hasOBONamespace>GAZ</oboInOwl:hasOBONamespace>
        <oboInOwl:id>GAZ:00041531</oboInOwl:id>
        <rdfs:label>Lake Rukwa</rdfs:label>
    </owl:NamedIndividual>
    


    <!-- http://purl.obolibrary.org/obo/GAZ_00041532 -->

    <owl:NamedIndividual rdf:about="http://purl.obolibrary.org/obo/GAZ_00041532">
        <obo:RO_0001025 rdf:resource="http://purl.obolibrary.org/obo/GAZ_00000007"/>
        <obo:IAO_0000115>An endorheic lake and swamp system in the Northern Province of Zambia. A rift valley lake lying in a branch of the Great Rift Valley, running from the Luapula River to Lake Tanganyika. There are some hot springs characteristics of a rift valley to the east. Its water is muddy in appearance, at times appearing reddish and &apos;slightly oily&apos;.</obo:IAO_0000115>
        <oboInOwl:hasOBONamespace>GAZ</oboInOwl:hasOBONamespace>
        <oboInOwl:id>GAZ:00041532</oboInOwl:id>
        <rdfs:label>Lake Mweru Wantipa</rdfs:label>
    </owl:NamedIndividual>
    


    <!-- http://purl.obolibrary.org/obo/GAZ_00041533 -->

    <owl:NamedIndividual rdf:about="http://purl.obolibrary.org/obo/GAZ_00041533">
        <obo:RO_0001025 rdf:resource="http://purl.obolibrary.org/obo/GAZ_00000007"/>
        <obo:IAO_0000115>A lake located in the western Great Rift Valley, on the border between the Democratic Republic of the Congo and Uganda, with its northern shore a few km south of the Equator. Lake Edward lies at an elevation of 920 metres, is 77 km long by 40 km wide at its maximum points, and covers a total surface area of 2,325 km2 (the 15th largest on the continent). The lake is fed by the Nyamugasani, the Ishasha, the Rutshuru, and the Rwindi rivers. It empties to the north via the Semliki River into Lake Albert. Lake George to the northeast empties into Lake Edward via the Kazinga Channel.</obo:IAO_0000115>
        <oboInOwl:hasOBONamespace>GAZ</oboInOwl:hasOBONamespace>
        <oboInOwl:id>GAZ:00041533</oboInOwl:id>
        <rdfs:label>Lake Edward</rdfs:label>
    </owl:NamedIndividual>
    


    <!-- http://purl.obolibrary.org/obo/GAZ_00041534 -->

    <owl:NamedIndividual rdf:about="http://purl.obolibrary.org/obo/GAZ_00041534">
        <obo:RO_0001025 rdf:resource="http://purl.obolibrary.org/obo/GAZ_00000007"/>
        <obo:IAO_0000115>A monomictic freshwater lake located in the center of the continent, on the border between Uganda and the Democratic Republic of the Congo (formerly Zaire). Lake Albert is the northernmost of the chain of lakes in the Great Rift Valley; it is about 160 km long and 30 km wide, with a maximum depth of 51 m, and a surface elevation of 619 m above sea level. Lake Albert is part of the complicated system of the upper Nile. Its main sources are the Victoria Nile, ultimately coming from Lake Victoria to the southeast, and the Semliki River, which issues from Lake Edward to the southwest. The water of the Victoria Nile is much less saline than that of Lake Albert. Its outlet, at the northernmost tip of the lake, is the Albert Nile (which becomes known as the Mountain Nile when it enters Sudan).</obo:IAO_0000115>
        <oboInOwl:hasOBONamespace>GAZ</oboInOwl:hasOBONamespace>
        <oboInOwl:id>GAZ:00041534</oboInOwl:id>
        <rdfs:label>Lake Albert</rdfs:label>
    </owl:NamedIndividual>
    


    <!-- http://purl.obolibrary.org/obo/GAZ_00041535 -->

    <owl:NamedIndividual rdf:about="http://purl.obolibrary.org/obo/GAZ_00041535">
        <rdf:type rdf:resource="http://purl.obolibrary.org/obo/ENVO_00000019"/>
        <obo:RO_0001025 rdf:resource="http://purl.obolibrary.org/obo/GAZ_00000007"/>
        <obo:IAO_0000115>A soda lake located in northern Tanzania, close to the Kenyan border, in Africa&apos;s Great Rift Valley. The lake is quite shallow, less than three m deep, and varies in width depending on its water level.</obo:IAO_0000115>
        <oboInOwl:hasOBONamespace>GAZ</oboInOwl:hasOBONamespace>
        <oboInOwl:id>GAZ:00041535</oboInOwl:id>
        <rdfs:label>Lake Natron</rdfs:label>
    </owl:NamedIndividual>
    


    <!-- http://purl.obolibrary.org/obo/GAZ_00041536 -->

    <owl:NamedIndividual rdf:about="http://purl.obolibrary.org/obo/GAZ_00041536">
        <obo:RO_0001025 rdf:resource="http://purl.obolibrary.org/obo/GAZ_00000007"/>
        <obo:RO_0001025 rdf:resource="http://purl.obolibrary.org/obo/GAZ_00136138"/>
        <obo:IAO_0000115>An endorheic soda lake located south of the Serengeti National Park and immediately southwest of the Ngorongoro Crater in the Crater Highlands area of Tanzania.</obo:IAO_0000115>
        <oboInOwl:hasOBONamespace>GAZ</oboInOwl:hasOBONamespace>
        <oboInOwl:id>GAZ:00041536</oboInOwl:id>
        <rdfs:label>Lake Eyasi</rdfs:label>
    </owl:NamedIndividual>
    


    <!-- http://purl.obolibrary.org/obo/GAZ_00041537 -->

    <owl:NamedIndividual rdf:about="http://purl.obolibrary.org/obo/GAZ_00041537">
        <obo:RO_0001025 rdf:resource="http://purl.obolibrary.org/obo/GAZ_00000007"/>
        <obo:IAO_0000115>A holopolymictic freshwater lake in Kenya, lying north west of Nairobi, outside the town of Naivasha. It is part of the Great Rift Valley. A Ramsar Site.</obo:IAO_0000115>
        <oboInOwl:hasOBONamespace>GAZ</oboInOwl:hasOBONamespace>
        <oboInOwl:id>GAZ:00041537</oboInOwl:id>
        <rdfs:label>Lake Naivasha</rdfs:label>
    </owl:NamedIndividual>
    


    <!-- http://purl.obolibrary.org/obo/GAZ_00041538 -->

    <owl:NamedIndividual rdf:about="http://purl.obolibrary.org/obo/GAZ_00041538">
        <obo:RO_0001025 rdf:resource="http://purl.obolibrary.org/obo/GAZ_00000007"/>
        <obo:IAO_0000115>A monomictic alkaline endorheic lake.</obo:IAO_0000115>
        <oboInOwl:hasOBONamespace>GAZ</oboInOwl:hasOBONamespace>
        <oboInOwl:id>GAZ:00041538</oboInOwl:id>
        <rdfs:label>Lake Turkana</rdfs:label>
    </owl:NamedIndividual>
    


    <!-- http://purl.obolibrary.org/obo/GAZ_00041539 -->

    <owl:NamedIndividual rdf:about="http://purl.obolibrary.org/obo/GAZ_00041539">
        <obo:RO_0001025 rdf:resource="http://purl.obolibrary.org/obo/GAZ_00000007"/>
        <obo:IAO_0000115>A freshwater lake fed by several rivers. It has no obvious outlet; the waters seep into lava. A Ramsar Site.</obo:IAO_0000115>
        <oboInOwl:hasOBONamespace>GAZ</oboInOwl:hasOBONamespace>
        <oboInOwl:id>GAZ:00041539</oboInOwl:id>
        <rdfs:label>Lake Baringo</rdfs:label>
    </owl:NamedIndividual>
    


    <!-- http://purl.obolibrary.org/obo/GAZ_00041540 -->

    <owl:NamedIndividual rdf:about="http://purl.obolibrary.org/obo/GAZ_00041540">
        <obo:RO_0001025 rdf:resource="http://purl.obolibrary.org/obo/GAZ_00000007"/>
        <obo:RO_0001025 rdf:resource="http://purl.obolibrary.org/obo/GAZ_00236097"/>
        <obo:IAO_0000115>A saline, alkaline lake that lies at the northern end of the arid Suguta Valley in the northern Kenya Rift. It is separated from Lake Turkana by the Barrier volcanic complex, a group of young volcanoes that last erupted during the late 19th Century or early 20th Century. Saline hot springs discharge on the northern shoreline of Lake Logipi and at Cathedral Rocks near its southern limit, and help to maintain water at times of extreme aridity. During the rainy season, the lake is also recharged from the Suguta River which flows northward along the Suguta Valley, periodically forming a temporary lake (Lake Alablab) that unites with Logipi.</obo:IAO_0000115>
        <oboInOwl:hasOBONamespace>GAZ</oboInOwl:hasOBONamespace>
        <oboInOwl:id>GAZ:00041540</oboInOwl:id>
        <rdfs:label>Lake Logipi</rdfs:label>
    </owl:NamedIndividual>
    


    <!-- http://purl.obolibrary.org/obo/GAZ_00041541 -->

    <owl:NamedIndividual rdf:about="http://purl.obolibrary.org/obo/GAZ_00041541">
        <obo:RO_0001025 rdf:resource="http://purl.obolibrary.org/obo/GAZ_00041539"/>
        <obo:IAO_0000115>An Island in the center of Lake Baringo SW of Korosi volcano consists of young basaltic scoria cones that cap a trachytic shield volcano. The volcano is the smallest in the northern part of the Kenya rift valley. N-S-trending faults cut the complex, producing west-facing scarps. Smaller islands to the north and south are faulted basaltic lava flows; Parmalok Island to the SW is a breached trachytic tuff cone that fed a small lava flow. Hot springs, boiling mud pools, and fumaroles are present along the faults on the NE peninsula of the island.</obo:IAO_0000115>
        <oboInOwl:hasOBONamespace>GAZ</oboInOwl:hasOBONamespace>
        <oboInOwl:id>GAZ:00041541</oboInOwl:id>
        <rdfs:label>Ol Kokwe Island</rdfs:label>
    </owl:NamedIndividual>
    


    <!-- http://purl.obolibrary.org/obo/GAZ_00041542 -->

    <owl:NamedIndividual rdf:about="http://purl.obolibrary.org/obo/GAZ_00041542">
        <obo:RO_0001025 rdf:resource="http://purl.obolibrary.org/obo/GAZ_00041538"/>
        <obo:IAO_0000115>The northernmost and smallest of three volcanic islands in the Lake Turkana. North Island is the summit of Kenya&apos;s northernmost rift valley volcano and is primarily composed of trachyandesitic-to-trachytic phreatomagmatic deposits from overlapping eroded tuff cones or tuff rings. The center of the island consists of a young tuff ring about 1 km in diameter nested inside an older tuff ring. Two fresh unvegetated lava flows that reach the lake shore from the central tuff ring form lava deltas at the northern and western sides of the island; the northern delta is about 900 m wide.</obo:IAO_0000115>
        <oboInOwl:hasOBONamespace>GAZ</oboInOwl:hasOBONamespace>
        <oboInOwl:id>GAZ:00041542</oboInOwl:id>
        <rdfs:label>North Island</rdfs:label>
    </owl:NamedIndividual>
    


    <!-- http://purl.obolibrary.org/obo/GAZ_00041543 -->

    <owl:NamedIndividual rdf:about="http://purl.obolibrary.org/obo/GAZ_00041543">
        <obo:RO_0001025 rdf:resource="http://purl.obolibrary.org/obo/GAZ_00041538"/>
        <obo:IAO_0000115>An island that occupies the middle of Lake Turkana and is composed of more than a dozen craters and cones, three of which are filled by small lakes. The two largest lakes partially fill craters up to a km wide and about 80 m deep whose floors lie near sea level. The highest point on the dominantly basaltic island reaches 550 m, about 170 m above the lake surface. An E-W-trending chain of small explosion craters cuts the eastern side of the 3 km wide island. Several small islands to the SE represent partially submerged crater rims, and other cones and lava plugs lie beneath the lake surface near the island.</obo:IAO_0000115>
        <oboInOwl:hasOBONamespace>GAZ</oboInOwl:hasOBONamespace>
        <oboInOwl:id>GAZ:00041543</oboInOwl:id>
        <rdfs:label>Central Island</rdfs:label>
    </owl:NamedIndividual>
    


    <!-- http://purl.obolibrary.org/obo/GAZ_00041544 -->

    <owl:NamedIndividual rdf:about="http://purl.obolibrary.org/obo/GAZ_00041544">
        <obo:RO_0001025 rdf:resource="http://purl.obolibrary.org/obo/GAZ_00041538"/>
        <obo:IAO_0000115>An island that contains numerous tuff cones. Fresh-looking lava flows, erupted from a N-S fissure extending the 11 km length of the island, form much of the eastern shoreline. South Island rises 320 m above the lake to a height of 800 m and is part of a volcanic horst that extends 10 km to the north beneath the lake surface.</obo:IAO_0000115>
        <oboInOwl:hasOBONamespace>GAZ</oboInOwl:hasOBONamespace>
        <oboInOwl:id>GAZ:00041544</oboInOwl:id>
        <rdfs:label>South Island</rdfs:label>
    </owl:NamedIndividual>
    


    <!-- http://purl.obolibrary.org/obo/GAZ_00041545 -->

    <owl:NamedIndividual rdf:about="http://purl.obolibrary.org/obo/GAZ_00041545">
        <obo:RO_0001025 rdf:resource="http://purl.obolibrary.org/obo/GAZ_00041530"/>
        <obo:IAO_0000115>An island in Lake Mweru.</obo:IAO_0000115>
        <oboInOwl:hasOBONamespace>GAZ</oboInOwl:hasOBONamespace>
        <oboInOwl:id>GAZ:00041545</oboInOwl:id>
        <rdfs:label>Kilwa Island</rdfs:label>
    </owl:NamedIndividual>
    


    <!-- http://purl.obolibrary.org/obo/GAZ_00041546 -->

    <owl:NamedIndividual rdf:about="http://purl.obolibrary.org/obo/GAZ_00041546">
        <obo:RO_0001025 rdf:resource="http://purl.obolibrary.org/obo/GAZ_00041530"/>
        <oboInOwl:hasOBONamespace>GAZ</oboInOwl:hasOBONamespace>
        <oboInOwl:id>GAZ:00041546</oboInOwl:id>
        <rdfs:label>Isokwe Island</rdfs:label>
    </owl:NamedIndividual>
    


    <!-- http://purl.obolibrary.org/obo/GAZ_00041547 -->

    <owl:NamedIndividual rdf:about="http://purl.obolibrary.org/obo/GAZ_00041547">
        <obo:RO_0001025 rdf:resource="http://purl.obolibrary.org/obo/GAZ_00041534"/>
        <oboInOwl:hasOBONamespace>GAZ</oboInOwl:hasOBONamespace>
        <oboInOwl:id>GAZ:00041547</oboInOwl:id>
        <rdfs:label>Rukwanzi Island</rdfs:label>
    </owl:NamedIndividual>
    


    <!-- http://purl.obolibrary.org/obo/GAZ_00041548 -->

    <owl:NamedIndividual rdf:about="http://purl.obolibrary.org/obo/GAZ_00041548">
        <obo:RO_0001025 rdf:resource="http://purl.obolibrary.org/obo/GAZ_00041537"/>
        <obo:IAO_0000115>An island of Lake Naivasha.</obo:IAO_0000115>
        <oboInOwl:hasOBONamespace>GAZ</oboInOwl:hasOBONamespace>
        <oboInOwl:id>GAZ:00041548</oboInOwl:id>
        <rdfs:label>Crescent Island</rdfs:label>
    </owl:NamedIndividual>
    


    <!-- http://purl.obolibrary.org/obo/GAZ_00041549 -->

    <owl:NamedIndividual rdf:about="http://purl.obolibrary.org/obo/GAZ_00041549">
        <obo:RO_0001025 rdf:resource="http://purl.obolibrary.org/obo/GAZ_00053591"/>
        <obo:IAO_0000115>A polymictic soda lake. A Ramsar Site.</obo:IAO_0000115>
        <oboInOwl:hasOBONamespace>GAZ</oboInOwl:hasOBONamespace>
        <oboInOwl:id>GAZ:00041549</oboInOwl:id>
        <rdfs:label>Lake Nakuru</rdfs:label>
    </owl:NamedIndividual>
    


    <!-- http://purl.obolibrary.org/obo/GAZ_00041550 -->

    <owl:NamedIndividual rdf:about="http://purl.obolibrary.org/obo/GAZ_00041550">
        <obo:RO_0001025 rdf:resource="http://purl.obolibrary.org/obo/GAZ_00000007"/>
        <obo:RO_0001025 rdf:resource="http://purl.obolibrary.org/obo/GAZ_00123543"/>
        <obo:IAO_0000115>A lake that is the source of the Blue Nile and is the largest lake in Ethiopia. Located in the north-western Ethiopian highlands. Lake Tana is fed by the Little Abay, Reb and Gumara Rivers.</obo:IAO_0000115>
        <oboInOwl:hasOBONamespace>GAZ</oboInOwl:hasOBONamespace>
        <oboInOwl:id>GAZ:00041550</oboInOwl:id>
        <rdfs:label>Lake Tana</rdfs:label>
    </owl:NamedIndividual>
    


    <!-- http://purl.obolibrary.org/obo/GAZ_00041551 -->

    <owl:NamedIndividual rdf:about="http://purl.obolibrary.org/obo/GAZ_00041551">
        <obo:RO_0001025 rdf:resource="http://purl.obolibrary.org/obo/GAZ_00041550"/>
        <obo:IAO_0000115>An island in Lake Tana in Ethiopia.</obo:IAO_0000115>
        <oboInOwl:hasOBONamespace>GAZ</oboInOwl:hasOBONamespace>
        <oboInOwl:id>GAZ:00041551</oboInOwl:id>
        <rdfs:label>Tana Qirqos Island</rdfs:label>
    </owl:NamedIndividual>
    


    <!-- http://purl.obolibrary.org/obo/GAZ_00041552 -->

    <owl:NamedIndividual rdf:about="http://purl.obolibrary.org/obo/GAZ_00041552">
        <obo:RO_0001025 rdf:resource="http://purl.obolibrary.org/obo/GAZ_00041550"/>
        <obo:IAO_0000115>An island of Lake Tana.</obo:IAO_0000115>
        <oboInOwl:hasOBONamespace>GAZ</oboInOwl:hasOBONamespace>
        <oboInOwl:id>GAZ:00041552</oboInOwl:id>
        <rdfs:label>Meshralia Island</rdfs:label>
    </owl:NamedIndividual>
    


    <!-- http://purl.obolibrary.org/obo/GAZ_00041553 -->

    <owl:NamedIndividual rdf:about="http://purl.obolibrary.org/obo/GAZ_00041553">
        <obo:RO_0001025 rdf:resource="http://purl.obolibrary.org/obo/GAZ_00041550"/>
        <obo:IAO_0000115>An island of Lake Tana.</obo:IAO_0000115>
        <oboInOwl:hasOBONamespace>GAZ</oboInOwl:hasOBONamespace>
        <oboInOwl:id>GAZ:00041553</oboInOwl:id>
        <rdfs:label>Daga Island</rdfs:label>
    </owl:NamedIndividual>
    


    <!-- http://purl.obolibrary.org/obo/GAZ_00041554 -->

    <owl:NamedIndividual rdf:about="http://purl.obolibrary.org/obo/GAZ_00041554">
        <obo:RO_0001025 rdf:resource="http://purl.obolibrary.org/obo/GAZ_00041550"/>
        <obo:IAO_0000115>The biggest island (approximately 16 km2) on Lake Tana in Ethiopia. It is administratively included in the Achefer woreda of the Mirab Gojjam Zone.</obo:IAO_0000115>
        <oboInOwl:hasOBONamespace>GAZ</oboInOwl:hasOBONamespace>
        <oboInOwl:id>GAZ:00041554</oboInOwl:id>
        <rdfs:label>Dek Island</rdfs:label>
    </owl:NamedIndividual>
    


    <!-- http://purl.obolibrary.org/obo/GAZ_00041555 -->

    <owl:NamedIndividual rdf:about="http://purl.obolibrary.org/obo/GAZ_00041555">
        <obo:RO_0001025 rdf:resource="http://purl.obolibrary.org/obo/GAZ_00000007"/>
        <obo:IAO_0000115>A freshwater Rift Valley lake of Ethiopia. It is located about 60 miles south of Addis Ababa, on the border between the regions (or kililoch) of Oromia and of the Southern Nations, Nationalities, and Peoples. The lake is fed primarily by two rivers, the Meki and the Katar, but does not always have an outflow, although in some years it drains into Lake Abijatta.</obo:IAO_0000115>
        <oboInOwl:hasOBONamespace>GAZ</oboInOwl:hasOBONamespace>
        <oboInOwl:id>GAZ:00041555</oboInOwl:id>
        <rdfs:label>Lake Zway</rdfs:label>
    </owl:NamedIndividual>
    


    <!-- http://purl.obolibrary.org/obo/GAZ_00041556 -->

    <owl:NamedIndividual rdf:about="http://purl.obolibrary.org/obo/GAZ_00041556">
        <obo:RO_0001025 rdf:resource="http://purl.obolibrary.org/obo/GAZ_00000007"/>
        <obo:IAO_0000115>A polymictic freshwater lake in Ethiopia, located in the Rift Valley south of Addis Ababa. Thought to have a subterranean outlet.</obo:IAO_0000115>
        <oboInOwl:hasOBONamespace>GAZ</oboInOwl:hasOBONamespace>
        <oboInOwl:id>GAZ:00041556</oboInOwl:id>
        <rdfs:label>Lake Awasa</rdfs:label>
    </owl:NamedIndividual>
    


    <!-- http://purl.obolibrary.org/obo/GAZ_00041557 -->

    <owl:NamedIndividual rdf:about="http://purl.obolibrary.org/obo/GAZ_00041557">
        <obo:RO_0001025 rdf:resource="http://purl.obolibrary.org/obo/GAZ_00000007"/>
        <obo:IAO_0000115>A lake in Ethiopia.</obo:IAO_0000115>
        <oboInOwl:hasOBONamespace>GAZ</oboInOwl:hasOBONamespace>
        <oboInOwl:id>GAZ:00041557</oboInOwl:id>
        <rdfs:label>Lake Koka</rdfs:label>
    </owl:NamedIndividual>
    


    <!-- http://purl.obolibrary.org/obo/GAZ_00041559 -->

    <owl:NamedIndividual rdf:about="http://purl.obolibrary.org/obo/GAZ_00041559">
        <obo:RO_0001025 rdf:resource="http://purl.obolibrary.org/obo/GAZ_00000007"/>
        <obo:IAO_0000115>An endorheic alkaline lake in Ethiopia south of Addis Ababa, in the Abijatta-Shalla National Park.</obo:IAO_0000115>
        <oboInOwl:hasOBONamespace>GAZ</oboInOwl:hasOBONamespace>
        <oboInOwl:id>GAZ:00041559</oboInOwl:id>
        <rdfs:label>Lake Abijatta</rdfs:label>
    </owl:NamedIndividual>
    


    <!-- http://purl.obolibrary.org/obo/GAZ_00041560 -->

    <owl:NamedIndividual rdf:about="http://purl.obolibrary.org/obo/GAZ_00041560">
        <obo:RO_0001025 rdf:resource="http://purl.obolibrary.org/obo/GAZ_00000007"/>
        <obo:IAO_0000115>A lake in the Southern Nations, Nationalities, and Peoples Region of Ethiopia. Located in the Great Rift Valley, east of the Guge Mountains. It is fed on its northern shore by the Bilate River, which rises on the southern slopes of Mount Gurage.</obo:IAO_0000115>
        <oboInOwl:hasOBONamespace>GAZ</oboInOwl:hasOBONamespace>
        <oboInOwl:id>GAZ:00041560</oboInOwl:id>
        <rdfs:label>Lake Abaya</rdfs:label>
    </owl:NamedIndividual>
    


    <!-- http://purl.obolibrary.org/obo/GAZ_00041561 -->

    <owl:NamedIndividual rdf:about="http://purl.obolibrary.org/obo/GAZ_00041561">
        <obo:RO_0001025 rdf:resource="http://purl.obolibrary.org/obo/GAZ_00041560"/>
        <oboInOwl:hasOBONamespace>GAZ</oboInOwl:hasOBONamespace>
        <oboInOwl:id>GAZ:00041561</oboInOwl:id>
        <rdfs:label>Aruro Island</rdfs:label>
    </owl:NamedIndividual>
    


    <!-- http://purl.obolibrary.org/obo/GAZ_00041562 -->

    <owl:NamedIndividual rdf:about="http://purl.obolibrary.org/obo/GAZ_00041562">
        <obo:RO_0001025 rdf:resource="http://purl.obolibrary.org/obo/GAZ_00041555"/>
        <obo:IAO_0000115>An island of Lake Zway.</obo:IAO_0000115>
        <oboInOwl:hasOBONamespace>GAZ</oboInOwl:hasOBONamespace>
        <oboInOwl:id>GAZ:00041562</oboInOwl:id>
        <rdfs:label>Galila Island</rdfs:label>
    </owl:NamedIndividual>
    


    <!-- http://purl.obolibrary.org/obo/GAZ_00041563 -->

    <owl:NamedIndividual rdf:about="http://purl.obolibrary.org/obo/GAZ_00041563">
        <obo:RO_0001025 rdf:resource="http://purl.obolibrary.org/obo/GAZ_00015452"/>
        <obo:IAO_0000115>An island in Lake Victoria.</obo:IAO_0000115>
        <oboInOwl:hasOBONamespace>GAZ</oboInOwl:hasOBONamespace>
        <oboInOwl:id>GAZ:00041563</oboInOwl:id>
        <rdfs:label>Lolui Island</rdfs:label>
    </owl:NamedIndividual>
    


    <!-- http://purl.obolibrary.org/obo/GAZ_00041564 -->

    <owl:NamedIndividual rdf:about="http://purl.obolibrary.org/obo/GAZ_00041564">
        <obo:RO_0001025 rdf:resource="http://purl.obolibrary.org/obo/GAZ_00041555"/>
        <obo:IAO_0000115>An island of Lake Zway.</obo:IAO_0000115>
        <oboInOwl:hasOBONamespace>GAZ</oboInOwl:hasOBONamespace>
        <oboInOwl:id>GAZ:00041564</oboInOwl:id>
        <rdfs:label>Tullu Gudo Island</rdfs:label>
    </owl:NamedIndividual>
    


    <!-- http://purl.obolibrary.org/obo/GAZ_00041565 -->

    <owl:NamedIndividual rdf:about="http://purl.obolibrary.org/obo/GAZ_00041565">
        <obo:RO_0001025 rdf:resource="http://purl.obolibrary.org/obo/GAZ_00041555"/>
        <obo:IAO_0000115>An island of Lake Zway.</obo:IAO_0000115>
        <oboInOwl:hasOBONamespace>GAZ</oboInOwl:hasOBONamespace>
        <oboInOwl:id>GAZ:00041565</oboInOwl:id>
        <rdfs:label>Bird Island</rdfs:label>
    </owl:NamedIndividual>
    


    <!-- http://purl.obolibrary.org/obo/GAZ_00041566 -->

    <owl:NamedIndividual rdf:about="http://purl.obolibrary.org/obo/GAZ_00041566">
        <obo:RO_0001025 rdf:resource="http://purl.obolibrary.org/obo/GAZ_00041555"/>
        <obo:IAO_0000115>An island of Lake Zway.</obo:IAO_0000115>
        <oboInOwl:hasOBONamespace>GAZ</oboInOwl:hasOBONamespace>
        <oboInOwl:id>GAZ:00041566</oboInOwl:id>
        <rdfs:label>Debre Sina Island</rdfs:label>
    </owl:NamedIndividual>
    


    <!-- http://purl.obolibrary.org/obo/GAZ_00041571 -->

    <owl:NamedIndividual rdf:about="http://purl.obolibrary.org/obo/GAZ_00041571">
        <obo:RO_0001025 rdf:resource="http://purl.obolibrary.org/obo/GAZ_00015452"/>
        <obo:IAO_0000115>An island in Lake Victoria.</obo:IAO_0000115>
        <oboInOwl:hasOBONamespace>GAZ</oboInOwl:hasOBONamespace>
        <oboInOwl:id>GAZ:00041571</oboInOwl:id>
        <rdfs:label>Iroba Island</rdfs:label>
    </owl:NamedIndividual>
    


    <!-- http://purl.obolibrary.org/obo/GAZ_00041572 -->

    <owl:NamedIndividual rdf:about="http://purl.obolibrary.org/obo/GAZ_00041572">
        <obo:RO_0001025 rdf:resource="http://purl.obolibrary.org/obo/GAZ_00052895"/>
        <obo:IAO_0000115>An island that lies in the eastern part of Lake Victoria, at the mouth of the Winam Gulf. Part of Kenya, it lies west of Rusinga Island.</obo:IAO_0000115>
        <oboInOwl:hasOBONamespace>GAZ</oboInOwl:hasOBONamespace>
        <oboInOwl:id>GAZ:00041572</oboInOwl:id>
        <rdfs:label>Mfangano Island</rdfs:label>
    </owl:NamedIndividual>
    


    <!-- http://purl.obolibrary.org/obo/GAZ_00041573 -->

    <owl:NamedIndividual rdf:about="http://purl.obolibrary.org/obo/GAZ_00041573">
        <obo:RO_0001025 rdf:resource="http://purl.obolibrary.org/obo/GAZ_00015452"/>
        <obo:IAO_0000115>An island in Lake Victoria.</obo:IAO_0000115>
        <oboInOwl:hasOBONamespace>GAZ</oboInOwl:hasOBONamespace>
        <oboInOwl:id>GAZ:00041573</oboInOwl:id>
        <rdfs:label>Ukara Island</rdfs:label>
    </owl:NamedIndividual>
    


    <!-- http://purl.obolibrary.org/obo/GAZ_00041574 -->

    <owl:NamedIndividual rdf:about="http://purl.obolibrary.org/obo/GAZ_00041574">
        <obo:RO_0001025 rdf:resource="http://purl.obolibrary.org/obo/GAZ_00015452"/>
        <obo:IAO_0000115>An island in Lake Victoria.</obo:IAO_0000115>
        <oboInOwl:hasOBONamespace>GAZ</oboInOwl:hasOBONamespace>
        <oboInOwl:id>GAZ:00041574</oboInOwl:id>
        <rdfs:label>Kome Island [South]</rdfs:label>
    </owl:NamedIndividual>
    


    <!-- http://purl.obolibrary.org/obo/GAZ_00041575 -->

    <owl:NamedIndividual rdf:about="http://purl.obolibrary.org/obo/GAZ_00041575">
        <obo:RO_0001025 rdf:resource="http://purl.obolibrary.org/obo/GAZ_00015452"/>
        <obo:IAO_0000115>A small island in Lake Victoria, Tanzania.</obo:IAO_0000115>
        <oboInOwl:hasOBONamespace>GAZ</oboInOwl:hasOBONamespace>
        <oboInOwl:id>GAZ:00041575</oboInOwl:id>
        <rdfs:label>Nabuyongo Island</rdfs:label>
    </owl:NamedIndividual>
    


    <!-- http://purl.obolibrary.org/obo/GAZ_00041576 -->

    <owl:NamedIndividual rdf:about="http://purl.obolibrary.org/obo/GAZ_00041576">
        <obo:RO_0001025 rdf:resource="http://purl.obolibrary.org/obo/GAZ_00015452"/>
        <obo:IAO_0000115>An island in Lake Victoria.</obo:IAO_0000115>
        <oboInOwl:hasOBONamespace>GAZ</oboInOwl:hasOBONamespace>
        <oboInOwl:id>GAZ:00041576</oboInOwl:id>
        <rdfs:label>Bumbire Island</rdfs:label>
    </owl:NamedIndividual>
    


    <!-- http://purl.obolibrary.org/obo/GAZ_00041577 -->

    <owl:NamedIndividual rdf:about="http://purl.obolibrary.org/obo/GAZ_00041577">
        <obo:RO_0001025 rdf:resource="http://purl.obolibrary.org/obo/GAZ_00015452"/>
        <obo:IAO_0000115>An island in Lake Victoria.</obo:IAO_0000115>
        <oboInOwl:hasOBONamespace>GAZ</oboInOwl:hasOBONamespace>
        <oboInOwl:id>GAZ:00041577</oboInOwl:id>
        <rdfs:label>Kome Island [North]</rdfs:label>
    </owl:NamedIndividual>
    


    <!-- http://purl.obolibrary.org/obo/GAZ_00041578 -->

    <owl:NamedIndividual rdf:about="http://purl.obolibrary.org/obo/GAZ_00041578">
        <obo:RO_0001025 rdf:resource="http://purl.obolibrary.org/obo/GAZ_00015452"/>
        <obo:IAO_0000115>An island in Lake Victoria.</obo:IAO_0000115>
        <oboInOwl:hasOBONamespace>GAZ</oboInOwl:hasOBONamespace>
        <oboInOwl:id>GAZ:00041578</oboInOwl:id>
        <rdfs:label>Ikuza Island</rdfs:label>
    </owl:NamedIndividual>
    


    <!-- http://purl.obolibrary.org/obo/GAZ_00041579 -->

    <owl:NamedIndividual rdf:about="http://purl.obolibrary.org/obo/GAZ_00041579">
        <obo:RO_0001025 rdf:resource="http://purl.obolibrary.org/obo/GAZ_00015452"/>
        <obo:IAO_0000115>An island that lies in the eastern part of Lake Victoria at the mouth of the Winam Gulf. Part of Kenya, it is linked to Mbita Point on the mainland by a causeway.</obo:IAO_0000115>
        <oboInOwl:hasOBONamespace>GAZ</oboInOwl:hasOBONamespace>
        <oboInOwl:id>GAZ:00041579</oboInOwl:id>
        <rdfs:label>Rusinga Island</rdfs:label>
    </owl:NamedIndividual>
    


    <!-- http://purl.obolibrary.org/obo/GAZ_00041580 -->

    <owl:NamedIndividual rdf:about="http://purl.obolibrary.org/obo/GAZ_00041580">
        <obo:RO_0001025 rdf:resource="http://purl.obolibrary.org/obo/GAZ_00052895"/>
        <obo:IAO_0000115>A small island (4.2 km2) in Winam Gulf of Lake Victoria in Kenya.</obo:IAO_0000115>
        <oboInOwl:hasOBONamespace>GAZ</oboInOwl:hasOBONamespace>
        <oboInOwl:id>GAZ:00041580</oboInOwl:id>
        <rdfs:label>Ndere Island</rdfs:label>
    </owl:NamedIndividual>
    


    <!-- http://purl.obolibrary.org/obo/GAZ_00041581 -->

    <owl:NamedIndividual rdf:about="http://purl.obolibrary.org/obo/GAZ_00041581">
        <obo:RO_0001025 rdf:resource="http://purl.obolibrary.org/obo/GAZ_00015452"/>
        <obo:IAO_0000115>An island in Lake Victoria.</obo:IAO_0000115>
        <oboInOwl:hasOBONamespace>GAZ</oboInOwl:hasOBONamespace>
        <oboInOwl:id>GAZ:00041581</oboInOwl:id>
        <rdfs:label>Bukasa Island</rdfs:label>
    </owl:NamedIndividual>
    


    <!-- http://purl.obolibrary.org/obo/GAZ_00041582 -->

    <owl:NamedIndividual rdf:about="http://purl.obolibrary.org/obo/GAZ_00041582">
        <obo:RO_0001025 rdf:resource="http://purl.obolibrary.org/obo/GAZ_00015452"/>
        <obo:IAO_0000115>A small island in northern Lake Victoria. It is about 10 km south of Kampala, Uganda.</obo:IAO_0000115>
        <oboInOwl:hasOBONamespace>GAZ</oboInOwl:hasOBONamespace>
        <oboInOwl:id>GAZ:00041582</oboInOwl:id>
        <rdfs:label>Bulingugwe Island</rdfs:label>
    </owl:NamedIndividual>
    


    <!-- http://purl.obolibrary.org/obo/GAZ_00044906 -->

    <owl:NamedIndividual rdf:about="http://purl.obolibrary.org/obo/GAZ_00044906">
        <obo:RO_0001025 rdf:resource="http://purl.obolibrary.org/obo/GAZ_00000007"/>
        <obo:IAO_0000115>A fertile valley in east Lebanon. Located about 30 km east of Beirut. The valley is situated between the Mount Lebanon to the west and the Anti-Lebanon mountain ranges to the east. It forms the northeasternmost extension of the Great Rift Valley, which stretches from Syria through the Red Sea into Africa. Beqaa Valley is about 120 km in length and has an average width of about 16 km.</obo:IAO_0000115>
        <oboInOwl:hasOBONamespace>GAZ</oboInOwl:hasOBONamespace>
        <oboInOwl:id>GAZ:00044906</oboInOwl:id>
        <rdfs:label>Beqaa Valley</rdfs:label>
    </owl:NamedIndividual>
    


    <!-- http://purl.obolibrary.org/obo/GAZ_00044911 -->

    <owl:NamedIndividual rdf:about="http://purl.obolibrary.org/obo/GAZ_00044911">
        <obo:RO_0001025 rdf:resource="http://purl.obolibrary.org/obo/GAZ_00248126"/>
        <obo:IAO_0000115>An endorheic saline lake in Southern Ethiopia on the boundary between the Oromia and the Southern Nations, Nationalities and Peoples&apos; Regions. When the lake is filled, it stretches into northern Kenya. Lying at the center of the Stephanie Wildlife Reserve, the lake measures some 40 miles by 15 miles. This lake is the southernmost and lowest (1,880 feet) of a series of lakes which lie in the north-easterly continuation of the Great Rift Valley; its watershed is separated from the watershed of Lake Turkana by the Humu Range and the hills south of it. The Kumbi Range rises on its eastern side. Chew Bahir is fed from the north by the Weito River, and its tributary the Galana Sagan. The Galana Sagan receives the overflow of Lake Chamo in some years, but no permanent connection exists.</obo:IAO_0000115>
        <oboInOwl:hasOBONamespace>GAZ</oboInOwl:hasOBONamespace>
        <oboInOwl:id>GAZ:00044911</oboInOwl:id>
        <rdfs:label>Lake Bahir</rdfs:label>
    </owl:NamedIndividual>
    


    <!-- http://purl.obolibrary.org/obo/GAZ_00044914 -->

    <owl:NamedIndividual rdf:about="http://purl.obolibrary.org/obo/GAZ_00044914">
        <obo:RO_0001025 rdf:resource="http://purl.obolibrary.org/obo/GAZ_00007520"/>
        <obo:IAO_0000115>A freshwater monomictic lake, being approximately 53 km in circumference, about 21 km long, and 13 km wide. The lake has a total area of 166 km2, and a maximum depth of approximately 43 m. It is situated deep in the Jordan Great Rift Valley, the valley caused by the separation of the African and Arabian Plates and is fed partly by underground springs although its main source is the Jordan River which flows through it from north to south. Consequently the area is subject to earthquakes and, in the past, volcanic activity. This is evidenced by the abundant basalt and other igneous rocks that define the geology of the Galilee region.</obo:IAO_0000115>
        <oboInOwl:hasOBONamespace>GAZ</oboInOwl:hasOBONamespace>
        <oboInOwl:id>GAZ:00044914</oboInOwl:id>
        <rdfs:label>Sea of Galilee</rdfs:label>
    </owl:NamedIndividual>
    


    <!-- http://purl.obolibrary.org/obo/GAZ_00044915 -->

    <owl:NamedIndividual rdf:about="http://purl.obolibrary.org/obo/GAZ_00044915">
        <obo:RO_0001025 rdf:resource="http://purl.obolibrary.org/obo/GAZ_00000007"/>
        <obo:IAO_0000115>A 375 km long strike-slip fault zone some 5 km wide in the north and 23 km wide in the south that forms part of the broader Great Rift Valley. Located in modern-day Israel, Jordan, the West Bank and the Golan Heights, this geographic region includes the Jordan River, Hula Valley, Lake Tiberias and the Dead Sea, features created by the physiographic and geologic process underway.</obo:IAO_0000115>
        <oboInOwl:hasOBONamespace>GAZ</oboInOwl:hasOBONamespace>
        <oboInOwl:id>GAZ:00044915</oboInOwl:id>
        <rdfs:label>Jordan Rift Valley</rdfs:label>
    </owl:NamedIndividual>
    


    <!-- http://purl.obolibrary.org/obo/GAZ_00044916 -->

    <owl:NamedIndividual rdf:about="http://purl.obolibrary.org/obo/GAZ_00044916">
        <obo:RO_0001025 rdf:resource="http://purl.obolibrary.org/obo/GAZ_00000007"/>
        <obo:RO_0001025 rdf:resource="http://purl.obolibrary.org/obo/GAZ_00044915"/>
        <obo:IAO_0000115>A section of the Great Rift Valley lying between the Dead Sea to the north and the Gulf of Aqaba or the Gulf of Eilat to the south. It forms part of the border between Israel to the west and Jordan to the east.</obo:IAO_0000115>
        <oboInOwl:hasOBONamespace>GAZ</oboInOwl:hasOBONamespace>
        <oboInOwl:id>GAZ:00044916</oboInOwl:id>
        <rdfs:label>Wadi Arabah</rdfs:label>
    </owl:NamedIndividual>
    


    <!-- http://purl.obolibrary.org/obo/GAZ_00049007 -->

    <owl:NamedIndividual rdf:about="http://purl.obolibrary.org/obo/GAZ_00049007">
        <obo:RO_0001025 rdf:resource="http://purl.obolibrary.org/obo/GAZ_00007862"/>
        <obo:IAO_0000115>The narrow sea passages, about 13 km wide, between the Sinai and Arabian peninsulas which separates the Gulf of Aqaba from the Red Sea.</obo:IAO_0000115>
        <oboInOwl:hasOBONamespace>GAZ</oboInOwl:hasOBONamespace>
        <oboInOwl:id>GAZ:00049007</oboInOwl:id>
        <rdfs:label>Straits of Tiran</rdfs:label>
    </owl:NamedIndividual>
    


    <!-- http://purl.obolibrary.org/obo/GAZ_00049008 -->

    <owl:NamedIndividual rdf:about="http://purl.obolibrary.org/obo/GAZ_00049008">
        <obo:RO_0001025 rdf:resource="http://purl.obolibrary.org/obo/GAZ_00049007"/>
        <obo:IAO_0000115>A Saudi Arabian island in the Straits of Tiran east of Tiran Island.</obo:IAO_0000115>
        <oboInOwl:hasOBONamespace>GAZ</oboInOwl:hasOBONamespace>
        <oboInOwl:id>GAZ:00049008</oboInOwl:id>
        <rdfs:label>Sanafir Island</rdfs:label>
    </owl:NamedIndividual>
    


    <!-- http://purl.obolibrary.org/obo/GAZ_00049009 -->

    <owl:NamedIndividual rdf:about="http://purl.obolibrary.org/obo/GAZ_00049009">
        <obo:RO_0001025 rdf:resource="http://purl.obolibrary.org/obo/GAZ_00049007"/>
        <obo:IAO_0000115>An island belonging to Saudi Arabia at the entrance of the Straits of Tiran, which separates the Red Sea and the Gulf of Aqaba.</obo:IAO_0000115>
        <oboInOwl:hasOBONamespace>GAZ</oboInOwl:hasOBONamespace>
        <oboInOwl:id>GAZ:00049009</oboInOwl:id>
        <rdfs:label>Tiran Island</rdfs:label>
    </owl:NamedIndividual>
    


    <!-- http://purl.obolibrary.org/obo/GAZ_00051205 -->

    <owl:NamedIndividual rdf:about="http://purl.obolibrary.org/obo/GAZ_00051205">
        <obo:RO_0001025 rdf:resource="http://purl.obolibrary.org/obo/GAZ_00000007"/>
        <obo:IAO_0000115>A geological depression in the Horn of Africa, where it overlaps Eritrea, the Afar Region of Ethiopia, and Djibouti. Only the Awash River flows into the depression, where it ends in a chain of lakes that increase in salinity.</obo:IAO_0000115>
        <oboInOwl:hasOBONamespace>GAZ</oboInOwl:hasOBONamespace>
        <oboInOwl:id>GAZ:00051205</oboInOwl:id>
        <rdfs:label>Afar Depression</rdfs:label>
    </owl:NamedIndividual>
    


    <!-- http://purl.obolibrary.org/obo/GAZ_00052497 -->

    <owl:NamedIndividual rdf:about="http://purl.obolibrary.org/obo/GAZ_00052497">
        <obo:RO_0001025 rdf:resource="http://purl.obolibrary.org/obo/GAZ_00031067"/>
        <obo:IAO_0000115>A port on the Red Sea coast of Eritrea.</obo:IAO_0000115>
        <oboInOwl:hasOBONamespace>GAZ</oboInOwl:hasOBONamespace>
        <oboInOwl:id>GAZ:00052497</oboInOwl:id>
        <rdfs:label>Massawa</rdfs:label>
    </owl:NamedIndividual>
    


    <!-- http://purl.obolibrary.org/obo/GAZ_00052498 -->

    <owl:NamedIndividual rdf:about="http://purl.obolibrary.org/obo/GAZ_00052498">
        <obo:RO_0001025 rdf:resource="http://purl.obolibrary.org/obo/GAZ_00000581"/>
        <obo:IAO_0000115>A river that flows from the Eritrean Highlands to the plains of Sudan. With a length of over 640 km, the Barka rises just outside Asmara, and flows in a northwestern direction through Agordat. It merges with the Anseba River near the border with Sudan.</obo:IAO_0000115>
        <oboInOwl:hasOBONamespace>GAZ</oboInOwl:hasOBONamespace>
        <oboInOwl:id>GAZ:00052498</oboInOwl:id>
        <rdfs:label>Barka River</rdfs:label>
    </owl:NamedIndividual>
    


    <!-- http://purl.obolibrary.org/obo/GAZ_00052499 -->

    <owl:NamedIndividual rdf:about="http://purl.obolibrary.org/obo/GAZ_00052499">
        <obo:RO_0001025 rdf:resource="http://purl.obolibrary.org/obo/GAZ_00230329"/>
        <obo:IAO_0000115>A monastery in the highlands of Eritrea near Keren in the Anseba Region.</obo:IAO_0000115>
        <oboInOwl:hasOBONamespace>GAZ</oboInOwl:hasOBONamespace>
        <oboInOwl:id>GAZ:00052499</oboInOwl:id>
        <rdfs:label>Debre Sina</rdfs:label>
    </owl:NamedIndividual>
    


    <!-- http://purl.obolibrary.org/obo/GAZ_00052500 -->

    <owl:NamedIndividual rdf:about="http://purl.obolibrary.org/obo/GAZ_00052500">
        <obo:RO_0001025 rdf:resource="http://purl.obolibrary.org/obo/GAZ_00031066"/>
        <obo:IAO_0000115>A populated place.</obo:IAO_0000115>
        <oboInOwl:hasOBONamespace>GAZ</oboInOwl:hasOBONamespace>
        <oboInOwl:id>GAZ:00052500</oboInOwl:id>
        <rdfs:label>Kubkub</rdfs:label>
    </owl:NamedIndividual>
    


    <!-- http://purl.obolibrary.org/obo/GAZ_00052501 -->

    <owl:NamedIndividual rdf:about="http://purl.obolibrary.org/obo/GAZ_00052501">
        <rdf:type rdf:resource="http://purl.obolibrary.org/obo/ENVO_00000856"/>
        <obo:RO_0001025 rdf:resource="http://purl.obolibrary.org/obo/GAZ_00031060"/>
        <obo:IAO_0000115>A populated place. A town in western Eritrea, lying south east of Kassala in Sudan, on the Gash River.</obo:IAO_0000115>
        <oboInOwl:hasOBONamespace>GAZ</oboInOwl:hasOBONamespace>
        <oboInOwl:id>GAZ:00052501</oboInOwl:id>
        <rdfs:label>Teseney</rdfs:label>
    </owl:NamedIndividual>
    


    <!-- http://purl.obolibrary.org/obo/GAZ_00052530 -->

    <owl:NamedIndividual rdf:about="http://purl.obolibrary.org/obo/GAZ_00052530">
        <rdf:type rdf:resource="http://purl.obolibrary.org/obo/ENVO_00000856"/>
        <obo:RO_0001025 rdf:resource="http://purl.obolibrary.org/obo/GAZ_00052531"/>
        <obo:IAO_0000115>A populated place. A village in south-central Ethiopia. Located in the Bale Zone of the Oromia Region in the heart of the Bale Mountains.</obo:IAO_0000115>
        <oboInOwl:hasOBONamespace>GAZ</oboInOwl:hasOBONamespace>
        <oboInOwl:id>GAZ:00052530</oboInOwl:id>
        <rdfs:label>Dinsho</rdfs:label>
    </owl:NamedIndividual>
    


    <!-- http://purl.obolibrary.org/obo/GAZ_00052531 -->

    <owl:NamedIndividual rdf:about="http://purl.obolibrary.org/obo/GAZ_00052531">
        <rdf:type rdf:resource="http://purl.obolibrary.org/obo/ENVO_00000106"/>
        <obo:RO_0001025 rdf:resource="http://purl.obolibrary.org/obo/GAZ_00123544"/>
        <obo:IAO_0000115>A range of mountains in the Oromia Region of southeast Ethiopia, south of the Awash River. They include Tullu Demtu, the second-highest mountain in Ethiopia (4377 m), and Mount Batu (4307 m). The Web River, a tributary of the Jubba River, rises in these mountains east of Goba.</obo:IAO_0000115>
        <oboInOwl:hasOBONamespace>GAZ</oboInOwl:hasOBONamespace>
        <oboInOwl:id>GAZ:00052531</oboInOwl:id>
        <rdfs:label>Bale Mountains</rdfs:label>
    </owl:NamedIndividual>
    


    <!-- http://purl.obolibrary.org/obo/GAZ_00052532 -->

    <owl:NamedIndividual rdf:about="http://purl.obolibrary.org/obo/GAZ_00052532">
        <obo:RO_0001025 rdf:resource="http://purl.obolibrary.org/obo/GAZ_00052531"/>
        <obo:IAO_0000115>A national park in the Oromia Region of southeast Ethiopia. Created in 1970, this park covers about 2,200 km2 of the Bale Mountains to the west and southwest of Goba in the Bale Zone. Within its boundaries are some of the highest points in Ethiopia, which include Mount Batu. Bale Mountains contains three distinct ecoregions: the northern plains, bush and woods; the central Sanetti Plateau with an average elevation of over 4000 meters; and the southern Harenna Forest.</obo:IAO_0000115>
        <oboInOwl:hasOBONamespace>GAZ</oboInOwl:hasOBONamespace>
        <oboInOwl:id>GAZ:00052532</oboInOwl:id>
        <rdfs:label>Bale Mountains National Park</rdfs:label>
    </owl:NamedIndividual>
    


    <!-- http://purl.obolibrary.org/obo/GAZ_00052553 -->

    <owl:NamedIndividual rdf:about="http://purl.obolibrary.org/obo/GAZ_00052553">
        <obo:IAO_0000115>A river that rises in the central highlands of Ethiopia near Mount Qachen, from where it flows west, north, then west again, forming the westernmost border of Ethiopia and Eritrea. The river continues into northeastern Sudan, where at 14deg10minN, 36degE, the Tekeze joins the Atbarah River, the lower course of which is a tributary of the Nile. The Tekeze is perhaps the true upper course of the Atbarah, as the former follows the longer course prior to the confluence of the two rivers. The names of its main tributaries in Ethiopia from its source are: on the right bank Tahali, Meri, Sellare, Sullo, Arekwa, Gheoa, Wari, Firafira, Tocoro and Gumalo Rivers; on the left bank Nili, Balagas, Saha, Bembea, Ataba, Zarima, and Kwalema Rivers.</obo:IAO_0000115>
        <oboInOwl:hasOBONamespace>GAZ</oboInOwl:hasOBONamespace>
        <oboInOwl:id>GAZ:00052553</oboInOwl:id>
        <rdfs:label>Tekeze River</rdfs:label>
    </owl:NamedIndividual>
    


    <!-- http://purl.obolibrary.org/obo/GAZ_00052559 -->

    <owl:NamedIndividual rdf:about="http://purl.obolibrary.org/obo/GAZ_00052559">
        <rdf:type rdf:resource="http://purl.obolibrary.org/obo/ENVO_00000191"/>
        <obo:RO_0001025 rdf:resource="http://purl.obolibrary.org/obo/GAZ_00052532"/>
        <obo:IAO_0000115>A major landform in Ethopia within a portion of the Bale Mountains.</obo:IAO_0000115>
        <oboInOwl:hasOBONamespace>GAZ</oboInOwl:hasOBONamespace>
        <oboInOwl:id>GAZ:00052559</oboInOwl:id>
        <rdfs:label>Sanetti Plateau</rdfs:label>
    </owl:NamedIndividual>
    


    <!-- http://purl.obolibrary.org/obo/GAZ_00052567 -->

    <owl:NamedIndividual rdf:about="http://purl.obolibrary.org/obo/GAZ_00052567">
        <obo:IAO_0000115>A river of southern Ethiopia. Its course is entirely contained within the boundaries of Ethiopia, and empties into Lake Turkana on the border with Kenya. It is the principal stream of an endorheic drainage basin; the part that the Omo drains includes part of the western Oromia Region and the middle of the Southern Nations, Nationalities, and People&apos;s Region. This river rises in the Shewan highlands and is a perennial river. Its course is generally to the south, however with a major bend to the west at about 7deg N 37deg 30minE to about 36deg E where it turns south until 5deg 30min N where it makes a large S- bend then resumes its southernly course to Lake Turkana.</obo:IAO_0000115>
        <oboInOwl:hasOBONamespace>GAZ</oboInOwl:hasOBONamespace>
        <oboInOwl:id>GAZ:00052567</oboInOwl:id>
        <rdfs:label>Omo River</rdfs:label>
    </owl:NamedIndividual>
    


    <!-- http://purl.obolibrary.org/obo/GAZ_00052578 -->

    <owl:NamedIndividual rdf:about="http://purl.obolibrary.org/obo/GAZ_00052578">
        <obo:RO_0001025 rdf:resource="http://purl.obolibrary.org/obo/GAZ_00123543"/>
        <obo:IAO_0000115>Mountains in northern Ethiopia, north east of Gondar. The mountains consist of plateaux separated by valleys and rising to pinnacles. The tallest peak is Ras Dashen (4,543 m); other notable heights include Mounts Biuat (4,437 m) and Abba Yared (4,460 m).</obo:IAO_0000115>
        <oboInOwl:hasOBONamespace>GAZ</oboInOwl:hasOBONamespace>
        <oboInOwl:id>GAZ:00052578</oboInOwl:id>
        <rdfs:label>Semien Mountains</rdfs:label>
    </owl:NamedIndividual>
    


    <!-- http://purl.obolibrary.org/obo/GAZ_00052683 -->

    <owl:NamedIndividual rdf:about="http://purl.obolibrary.org/obo/GAZ_00052683">
        <obo:RO_0001025 rdf:resource="http://purl.obolibrary.org/obo/GAZ_00051205"/>
        <obo:IAO_0000115>A saline lake in the northern end of the Afar Depression, Ethiopia.</obo:IAO_0000115>
        <oboInOwl:hasOBONamespace>GAZ</oboInOwl:hasOBONamespace>
        <oboInOwl:id>GAZ:00052683</oboInOwl:id>
        <rdfs:label>Lake Karum</rdfs:label>
    </owl:NamedIndividual>
    


    <!-- http://purl.obolibrary.org/obo/GAZ_00052684 -->

    <owl:NamedIndividual rdf:about="http://purl.obolibrary.org/obo/GAZ_00052684">
        <obo:RO_0001025 rdf:resource="http://purl.obolibrary.org/obo/GAZ_00051205"/>
        <obo:IAO_0000115>A saline crater lake in central Djibouti, located at the southern border of Tadjoura Region, touching Dikhil Region. Fed by subterranean inflows which include infiltration of sea water, as well as by wadis which lead into the depression.</obo:IAO_0000115>
        <oboInOwl:hasOBONamespace>GAZ</oboInOwl:hasOBONamespace>
        <oboInOwl:id>GAZ:00052684</oboInOwl:id>
        <rdfs:label>Lake Asal</rdfs:label>
    </owl:NamedIndividual>
    


    <!-- http://purl.obolibrary.org/obo/GAZ_00052883 -->

    <owl:NamedIndividual rdf:about="http://purl.obolibrary.org/obo/GAZ_00052883">
        <obo:IAO_0000115>A dam on the Yarmuk River.</obo:IAO_0000115>
        <oboInOwl:hasOBONamespace>GAZ</oboInOwl:hasOBONamespace>
        <oboInOwl:id>GAZ:00052883</oboInOwl:id>
        <rdfs:label>Maqarin Dam</rdfs:label>
    </owl:NamedIndividual>
    


    <!-- http://purl.obolibrary.org/obo/GAZ_00052895 -->

    <owl:NamedIndividual rdf:about="http://purl.obolibrary.org/obo/GAZ_00052895">
        <obo:RO_0001025 rdf:resource="http://purl.obolibrary.org/obo/GAZ_00015452"/>
        <obo:IAO_0000115>A significant extension of northeastern Lake Victoria into western Kenya. It is a shallow inlet and is connected to the main lake by Rusinga Channel (3 mi wide), which is partly masked from the main body of the lake by islands. The port of Kisumu, Kenya&apos;s fourth largest city, stands on its northeastern shore.</obo:IAO_0000115>
        <oboInOwl:hasOBONamespace>GAZ</oboInOwl:hasOBONamespace>
        <oboInOwl:id>GAZ:00052895</oboInOwl:id>
        <rdfs:label>Winam Gulf</rdfs:label>
    </owl:NamedIndividual>
    


    <!-- http://purl.obolibrary.org/obo/GAZ_00052896 -->

    <owl:NamedIndividual rdf:about="http://purl.obolibrary.org/obo/GAZ_00052896">
        <obo:RO_0001025 rdf:resource="http://purl.obolibrary.org/obo/GAZ_00052895"/>
        <oboInOwl:hasOBONamespace>GAZ</oboInOwl:hasOBONamespace>
        <oboInOwl:id>GAZ:00052896</oboInOwl:id>
        <rdfs:label>Asembo Bay</rdfs:label>
    </owl:NamedIndividual>
    


    <!-- http://purl.obolibrary.org/obo/GAZ_00052899 -->

    <owl:NamedIndividual rdf:about="http://purl.obolibrary.org/obo/GAZ_00052899">
        <obo:RO_0001025 rdf:resource="http://purl.obolibrary.org/obo/GAZ_00007523"/>
        <oboInOwl:hasOBONamespace>GAZ</oboInOwl:hasOBONamespace>
        <oboInOwl:id>GAZ:00052899</oboInOwl:id>
        <rdfs:label>Causeway Pond</rdfs:label>
    </owl:NamedIndividual>
    


    <!-- http://purl.obolibrary.org/obo/GAZ_00052911 -->

    <owl:NamedIndividual rdf:about="http://purl.obolibrary.org/obo/GAZ_00052911">
        <obo:RO_0001025 rdf:resource="http://purl.obolibrary.org/obo/GAZ_00052895"/>
        <obo:IAO_0000115>A bay on the south shore of Winam Gulf of Lake Victoria, in western Kenya.</obo:IAO_0000115>
        <oboInOwl:hasOBONamespace>GAZ</oboInOwl:hasOBONamespace>
        <oboInOwl:id>GAZ:00052911</oboInOwl:id>
        <rdfs:label>Homa Bay</rdfs:label>
    </owl:NamedIndividual>
    


    <!-- http://purl.obolibrary.org/obo/GAZ_00052985 -->

    <owl:NamedIndividual rdf:about="http://purl.obolibrary.org/obo/GAZ_00052985">
        <obo:RO_0001025 rdf:resource="http://purl.obolibrary.org/obo/GAZ_00000007"/>
        <oboInOwl:hasOBONamespace>GAZ</oboInOwl:hasOBONamespace>
        <oboInOwl:id>GAZ:00052985</oboInOwl:id>
        <rdfs:label>Laikipia Plateau</rdfs:label>
    </owl:NamedIndividual>
    


    <!-- http://purl.obolibrary.org/obo/GAZ_00052986 -->

    <owl:NamedIndividual rdf:about="http://purl.obolibrary.org/obo/GAZ_00052986">
        <obo:RO_0001025 rdf:resource="http://purl.obolibrary.org/obo/GAZ_00052985"/>
        <obo:IAO_0000115>A research center.</obo:IAO_0000115>
        <oboInOwl:hasOBONamespace>GAZ</oboInOwl:hasOBONamespace>
        <oboInOwl:id>GAZ:00052986</oboInOwl:id>
        <rdfs:label>Mpala Research Centre</rdfs:label>
    </owl:NamedIndividual>
    


    <!-- http://purl.obolibrary.org/obo/GAZ_00053546 -->

    <owl:NamedIndividual rdf:about="http://purl.obolibrary.org/obo/GAZ_00053546">
        <obo:RO_0001025 rdf:resource="http://purl.obolibrary.org/obo/GAZ_00000007"/>
        <obo:IAO_0000115>A volcanic complex separates Lake Turkana from the broad Suguta Trough to the south, the site of a former lake. The volcano is comprised of four overlapping shield volcanoes, with the youngest, Kakorinya, located over the axis of the East African Rift. Kalolenyang volcano lies west of Kakorinya, and Likaiu West and Likaiu East volcano are located to the ENE. A 3.8 km wide summit caldera was formed at Kakorinya volcano about 92,000 years ago. Youthful-looking trachytic and phonolitic lava domes and flows erupted within the caldera and along its ring fracture fill much of the caldera floor. Early Holocene fissure-related scoria cones and lava flows dot the volcano&apos;s southern and northern flanks. Solfataric fields are located within the caldera and on the western and southern flanks of the volcano.</obo:IAO_0000115>
        <oboInOwl:hasOBONamespace>GAZ</oboInOwl:hasOBONamespace>
        <oboInOwl:id>GAZ:00053546</oboInOwl:id>
        <rdfs:label>The Barrier Volcanic Complex</rdfs:label>
    </owl:NamedIndividual>
    


    <!-- http://purl.obolibrary.org/obo/GAZ_00053547 -->

    <owl:NamedIndividual rdf:about="http://purl.obolibrary.org/obo/GAZ_00053547">
        <obo:RO_0001025 rdf:resource="http://purl.obolibrary.org/obo/GAZ_00053546"/>
        <obo:IAO_0000115>A volcano in the Barrier Complex.</obo:IAO_0000115>
        <oboInOwl:hasOBONamespace>GAZ</oboInOwl:hasOBONamespace>
        <oboInOwl:id>GAZ:00053547</oboInOwl:id>
        <rdfs:label>Kakorinya Volcano</rdfs:label>
    </owl:NamedIndividual>
    


    <!-- http://purl.obolibrary.org/obo/GAZ_00053548 -->

    <owl:NamedIndividual rdf:about="http://purl.obolibrary.org/obo/GAZ_00053548">
        <obo:RO_0001025 rdf:resource="http://purl.obolibrary.org/obo/GAZ_00053546"/>
        <obo:IAO_0000115>A volcano in the Barrier Complex.</obo:IAO_0000115>
        <oboInOwl:hasOBONamespace>GAZ</oboInOwl:hasOBONamespace>
        <oboInOwl:id>GAZ:00053548</oboInOwl:id>
        <rdfs:label>Likaiu East Volcano</rdfs:label>
    </owl:NamedIndividual>
    


    <!-- http://purl.obolibrary.org/obo/GAZ_00053549 -->

    <owl:NamedIndividual rdf:about="http://purl.obolibrary.org/obo/GAZ_00053549">
        <obo:RO_0001025 rdf:resource="http://purl.obolibrary.org/obo/GAZ_00053546"/>
        <obo:IAO_0000115>A volcano in the Barrier Complex.</obo:IAO_0000115>
        <oboInOwl:hasOBONamespace>GAZ</oboInOwl:hasOBONamespace>
        <oboInOwl:id>GAZ:00053549</oboInOwl:id>
        <rdfs:label>Kakorinya Volcano</rdfs:label>
    </owl:NamedIndividual>
    


    <!-- http://purl.obolibrary.org/obo/GAZ_00053550 -->

    <owl:NamedIndividual rdf:about="http://purl.obolibrary.org/obo/GAZ_00053550">
        <obo:RO_0001025 rdf:resource="http://purl.obolibrary.org/obo/GAZ_00053546"/>
        <obo:IAO_0000115>A volcano in the Barrier Complex.</obo:IAO_0000115>
        <oboInOwl:hasOBONamespace>GAZ</oboInOwl:hasOBONamespace>
        <oboInOwl:id>GAZ:00053550</oboInOwl:id>
        <rdfs:label>Likaiu West Volcano</rdfs:label>
    </owl:NamedIndividual>
    


    <!-- http://purl.obolibrary.org/obo/GAZ_00053551 -->

    <owl:NamedIndividual rdf:about="http://purl.obolibrary.org/obo/GAZ_00053551">
        <obo:RO_0001025 rdf:resource="http://purl.obolibrary.org/obo/GAZ_00000007"/>
        <obo:IAO_0000115>A trachytic shield volcano is topped by parasitic cones and lava flows of upper Pleistocene and Holocene age. Voluminous basaltic effusive and explosive activity took place during the early Holocene on the lower northern, eastern, and southern flanks along the axis of the East African Rift, producing fissure-controlled subaerial basaltic scoria cones and lava flows, and partially or completely sublacustral tuff cones, tuff rings, and pillow lavas. Fluid olivine basalts were also erupted from a breached scoria cone forming the summit of Namarunu.</obo:IAO_0000115>
        <oboInOwl:hasOBONamespace>GAZ</oboInOwl:hasOBONamespace>
        <oboInOwl:id>GAZ:00053551</oboInOwl:id>
        <rdfs:label>Namarunu Volcano</rdfs:label>
    </owl:NamedIndividual>
    


    <!-- http://purl.obolibrary.org/obo/GAZ_00053554 -->

    <owl:NamedIndividual rdf:about="http://purl.obolibrary.org/obo/GAZ_00053554">
        <obo:RO_0001025 rdf:resource="http://purl.obolibrary.org/obo/GAZ_00000007"/>
        <obo:IAO_0000115>A shield volcano is situated at a narrow constriction in the Rift Valley and almost completely straddles it. A 5 x 3.5 km summit caldera formed about 38,000 years ago. Since then trachytic and basaltic lava flows were erupted on the northern and southern flanks and within the caldera. A NNE-SSW-trending chain of lake-filled basaltic maars extends along the floor of the rift from the lower flanks of the volcano. Young lava flows were also erupted from vents along rift valley faults. Well-preserved parasitic cones erupted along rift-parallel faults cutting the volcano abound; the latest eruption produced a trachytic lava flow dated from secular magnetic variation measurements at about the beginning of the 20th century. Fumarolic activity and hot steaming ground occurs along NNE-trending fissures within the caldera and along the lower NW flanks.</obo:IAO_0000115>
        <oboInOwl:hasOBONamespace>GAZ</oboInOwl:hasOBONamespace>
        <oboInOwl:id>GAZ:00053554</oboInOwl:id>
        <rdfs:label>Emuruangogolak Volcano</rdfs:label>
    </owl:NamedIndividual>
    


    <!-- http://purl.obolibrary.org/obo/GAZ_00053555 -->

    <owl:NamedIndividual rdf:about="http://purl.obolibrary.org/obo/GAZ_00053555">
        <obo:RO_0001025 rdf:resource="http://purl.obolibrary.org/obo/GAZ_00000007"/>
        <obo:IAO_0000115>A trachytic shield volcano, the largest Quaternary volcano in the northern Gregory Rift, completely straddles the East African Rift. An impressive 5 x 8 km summit caldera with 300 m deep walls is thought to have formed about 63,000 years ago. Caldera formation is thought to have been incremental, related to eruption of the Kantenmening basaltic and trachytic lava flows. A series of summit-area lava benches formed by eruptions from circumferential fissures has produced a volcano morphologically similar to Galapagos Islands volcanoes. Northern, eastern, and southern flanks are cut by a prominent broad rift zone 10 km wide and 30 km long, dotted with numerous pyroclastic cones. Lava domes on the upper eastern flank formed during the late Pleistocene and early Holocene, until about 7 ka. Youthful parasitic cones abound on the caldera floor and on the northern and NE flanks; the youngest lava flows may be little more than a few hundred years old (Williams et al. 1984). Geothermal activity occurs within the caldera and on the upper eastern flanks.</obo:IAO_0000115>
        <oboInOwl:hasOBONamespace>GAZ</oboInOwl:hasOBONamespace>
        <oboInOwl:id>GAZ:00053555</oboInOwl:id>
        <rdfs:label>Silali Volcano</rdfs:label>
    </owl:NamedIndividual>
    


    <!-- http://purl.obolibrary.org/obo/GAZ_00053556 -->

    <owl:NamedIndividual rdf:about="http://purl.obolibrary.org/obo/GAZ_00053556">
        <obo:RO_0001025 rdf:resource="http://purl.obolibrary.org/obo/GAZ_00000007"/>
        <obo:IAO_0000115>A shield volcano in the Gregory Rift contains a small 1.5 km wide summit caldera. Eruption of large volumes of trachytic pyroclastic rocks around the end of the Pleistocene and the beginning of the Holocene formed a NW-trending ridge of pyroclastic cones across the summit region; collapse of this area formed the summit caldera and associated craters. A second large crater SE of the caldera is 0.5 x 1 km wide and contains a pumice cone. The summit caldera is narrowly breached on the north side, which has funneled post-caldera lava flows in this direction. The three youngest post-caldera pyroclastic cones on the NE flank may be only a few hundred years old. A series of viscous trachytic lava flows were erupted from vents on the volcano&apos;s lower flanks. Young fissure-fed basalts were also erupted to the south, between Paka and Korosi volcanoes. Surficial geothermal activity is widespread at Paka both within the summit caldera and on extensive portions of the northern flank.</obo:IAO_0000115>
        <oboInOwl:hasOBONamespace>GAZ</oboInOwl:hasOBONamespace>
        <oboInOwl:id>GAZ:00053556</oboInOwl:id>
        <rdfs:label>Paka Volcano</rdfs:label>
    </owl:NamedIndividual>
    


    <!-- http://purl.obolibrary.org/obo/GAZ_00053557 -->

    <owl:NamedIndividual rdf:about="http://purl.obolibrary.org/obo/GAZ_00053557">
        <obo:RO_0001025 rdf:resource="http://purl.obolibrary.org/obo/GAZ_00000007"/>
        <obo:IAO_0000115>A broad shield volcano west of Lake Bogoria that has been cut by spectacular grid faults along the west margin of the Gregory Rift. Geysers on the west margin of Lake Bogoria may be of tectonic origin.</obo:IAO_0000115>
        <oboInOwl:hasOBONamespace>GAZ</oboInOwl:hasOBONamespace>
        <oboInOwl:id>GAZ:00053557</oboInOwl:id>
        <rdfs:label>Bogoria Volcano</rdfs:label>
    </owl:NamedIndividual>
    


    <!-- http://purl.obolibrary.org/obo/GAZ_00053558 -->

    <owl:NamedIndividual rdf:about="http://purl.obolibrary.org/obo/GAZ_00053558">
        <obo:RO_0001025 rdf:resource="http://purl.obolibrary.org/obo/GAZ_00000007"/>
        <obo:IAO_0000115>A shield volcano that lies at the north end of Lake Baringo. Unlike other rift valley volcanoes, it does not contain a summit caldera. Lava domes on the northern flanks have fed trachytic lava flows. The major stage of Korosi volcanism spanned a period between 0.4 and 0.1 million years ago and included the eruption of voluminous fluid basaltic lava flows and pyroclastic cone formation along a NNE-trending fissure cutting across the axis of the shield volcano. This was followed by the eruption of trachytic lava domes and pumice/scoria cones. The youngest activity, consisting of fissure-fed basaltic lava flows on the lower northern flanks between Korosi and Paka, was probably coeval with the latest eruptions on Ol Kokwe to the south, which are only a few hundred to a few thousand years old (Dunkley et al. 1993). Fumaroles and hot steaming ground occur around the summit cones and NW flanks over an area of 30 sq km.</obo:IAO_0000115>
        <oboInOwl:hasOBONamespace>GAZ</oboInOwl:hasOBONamespace>
        <oboInOwl:id>GAZ:00053558</oboInOwl:id>
        <rdfs:label>Korosi Volcano</rdfs:label>
    </owl:NamedIndividual>
    


    <!-- http://purl.obolibrary.org/obo/GAZ_00053560 -->

    <owl:NamedIndividual rdf:about="http://purl.obolibrary.org/obo/GAZ_00053560">
        <obo:RO_0001025 rdf:resource="http://purl.obolibrary.org/obo/GAZ_00000007"/>
        <obo:IAO_0000115>A shield volcano that occupies the floor of the East African Rift. Construction of a 30 cu km shield volcano beginning about 200,000 years ago was followed by the eruption of two voluminous ash-flow tuffs, each preceded by major pumice falls.</obo:IAO_0000115>
        <oboInOwl:hasOBONamespace>GAZ</oboInOwl:hasOBONamespace>
        <oboInOwl:id>GAZ:00053560</oboInOwl:id>
        <rdfs:label>Menengai Volcano</rdfs:label>
    </owl:NamedIndividual>
    


    <!-- http://purl.obolibrary.org/obo/GAZ_00053565 -->

    <owl:NamedIndividual rdf:about="http://purl.obolibrary.org/obo/GAZ_00053565">
        <obo:RO_0001025 rdf:resource="http://purl.obolibrary.org/obo/GAZ_00000007"/>
        <obo:IAO_0000115>A volcanic field located between Lake Elmenteita and Eburru volcano, is an area of pyroclastic cones and lava flows of varying ages.</obo:IAO_0000115>
        <oboInOwl:hasOBONamespace>GAZ</oboInOwl:hasOBONamespace>
        <oboInOwl:id>GAZ:00053565</oboInOwl:id>
        <rdfs:label>Elmenteita Badlands</rdfs:label>
    </owl:NamedIndividual>
    


    <!-- http://purl.obolibrary.org/obo/GAZ_00053566 -->

    <owl:NamedIndividual rdf:about="http://purl.obolibrary.org/obo/GAZ_00053566">
        <obo:RO_0001025 rdf:resource="http://purl.obolibrary.org/obo/GAZ_00000007"/>
        <obo:IAO_0000115>A comple volcano that is elongated perpendicular to the Gregory Rift NW of Lake Naivasha. The 2856 m high, E-W-trending main edifice is eroded, but young partly vegetated rhyolitic domes occur on the east flank and are probably of Holocene age A prominent late-Pleistocene rhyolitic lava flow from a SE-flank vents extends almost to Lake Naivasha. Extensive fumarolic activity occurs at cinder cones and craters constructed along dominantly N-S-trending faults cutting the massif.</obo:IAO_0000115>
        <oboInOwl:hasOBONamespace>GAZ</oboInOwl:hasOBONamespace>
        <oboInOwl:id>GAZ:00053566</oboInOwl:id>
        <rdfs:label>Ol Doinyo Eburru Volcanic Complex</rdfs:label>
    </owl:NamedIndividual>
    


    <!-- http://purl.obolibrary.org/obo/GAZ_00053567 -->

    <owl:NamedIndividual rdf:about="http://purl.obolibrary.org/obo/GAZ_00053567">
        <obo:RO_0001025 rdf:resource="http://purl.obolibrary.org/obo/GAZ_00000007"/>
        <obo:IAO_0000115>A volcanic complex, located immediately south of Lake Naivasha and west of Longonot volcano, comprises up to 80 individual commenditic and other peralkaline rhyolitic centers. A thick, geochemically diverse basal complex is overlain by a dominantly silicic lava-dome and lava-flow complex active from about 20,000 years ago to the present. The youngest known eruption originated from the Ololbutot fissure on the SE side of the complex produced lava flows and a pumice flow and has a radiocarbon age of about 180 years. Fumarolic activity occurs at the Njorowa Gorge and at the Orengingnai and Olkaria (Orgaria) pumice cones.</obo:IAO_0000115>
        <oboInOwl:hasOBONamespace>GAZ</oboInOwl:hasOBONamespace>
        <oboInOwl:id>GAZ:00053567</oboInOwl:id>
        <rdfs:label>Olkaria Volcanic Complex</rdfs:label>
    </owl:NamedIndividual>
    


    <!-- http://purl.obolibrary.org/obo/GAZ_00053568 -->

    <owl:NamedIndividual rdf:about="http://purl.obolibrary.org/obo/GAZ_00053568">
        <obo:RO_0001025 rdf:resource="http://purl.obolibrary.org/obo/GAZ_00053569"/>
        <obo:IAO_0000115>A stratovolcano SE of Lake Naivasha in the Gregory Rift valley contains a 8 x 12 km caldera. Formation of the caldera accompanied large explosive eruptions about 21,000 years ago. A large central cone that was constructed within the caldera forms the 2776 m high summit of the volcano. The younger cone is truncated by a circular, 1.8 km wide crater. Post-caldera lavas are found on the caldera floor and the volcano&apos;s flanks, marking a late stage of effusive eruptions. A well-preserved satellitic cone is located on the NE flank.</obo:IAO_0000115>
        <oboInOwl:hasOBONamespace>GAZ</oboInOwl:hasOBONamespace>
        <oboInOwl:id>GAZ:00053568</oboInOwl:id>
        <rdfs:label>Mount Longonot</rdfs:label>
    </owl:NamedIndividual>
    


    <!-- http://purl.obolibrary.org/obo/GAZ_00053569 -->

    <owl:NamedIndividual rdf:about="http://purl.obolibrary.org/obo/GAZ_00053569">
        <obo:RO_0001025 rdf:resource="http://purl.obolibrary.org/obo/GAZ_00000007"/>
        <oboInOwl:hasOBONamespace>GAZ</oboInOwl:hasOBONamespace>
        <oboInOwl:id>GAZ:00053569</oboInOwl:id>
        <rdfs:label>Mount Longonot National Park</rdfs:label>
    </owl:NamedIndividual>
    


    <!-- http://purl.obolibrary.org/obo/GAZ_00053570 -->

    <owl:NamedIndividual rdf:about="http://purl.obolibrary.org/obo/GAZ_00053570">
        <obo:RO_0001025 rdf:resource="http://purl.obolibrary.org/obo/GAZ_00000007"/>
        <obo:IAO_0000115>A caldera of the Kenya rift, Suswa contains a prominent lava cone on the south side of its 8 x 12 km caldera. Suswa lies south of Longonot volcano and about 50 km WNW of the capital city of Nairobi. Construction of an early shield volcano was followed by eruption of voluminous Pleistocene pumice flows and lava flows that accompanied incremental formation of the caldera.</obo:IAO_0000115>
        <oboInOwl:hasOBONamespace>GAZ</oboInOwl:hasOBONamespace>
        <oboInOwl:id>GAZ:00053570</oboInOwl:id>
        <rdfs:label>Suswa Volcano</rdfs:label>
    </owl:NamedIndividual>
    


    <!-- http://purl.obolibrary.org/obo/GAZ_00053571 -->

    <owl:NamedIndividual rdf:about="http://purl.obolibrary.org/obo/GAZ_00053571">
        <obo:RO_0001025 rdf:resource="http://purl.obolibrary.org/obo/GAZ_00053570"/>
        <obo:IAO_0000115>A post-caldera lava cone.</obo:IAO_0000115>
        <oboInOwl:hasOBONamespace>GAZ</oboInOwl:hasOBONamespace>
        <oboInOwl:id>GAZ:00053571</oboInOwl:id>
        <rdfs:label>Ol Doinyo Onyoke</rdfs:label>
    </owl:NamedIndividual>
    


    <!-- http://purl.obolibrary.org/obo/GAZ_00053591 -->

    <owl:NamedIndividual rdf:about="http://purl.obolibrary.org/obo/GAZ_00053591">
        <obo:RO_0001025 rdf:resource="http://purl.obolibrary.org/obo/GAZ_00000007"/>
        <obo:IAO_0000115>A national park that protects Lake Nakuru, near Nakuru Town.</obo:IAO_0000115>
        <oboInOwl:hasOBONamespace>GAZ</oboInOwl:hasOBONamespace>
        <oboInOwl:id>GAZ:00053591</oboInOwl:id>
        <rdfs:label>Lake Nakuru National Park</rdfs:label>
    </owl:NamedIndividual>
    


    <!-- http://purl.obolibrary.org/obo/GAZ_00053598 -->

    <owl:NamedIndividual rdf:about="http://purl.obolibrary.org/obo/GAZ_00053598">
        <obo:RO_0001025 rdf:resource="http://purl.obolibrary.org/obo/GAZ_00051205"/>
        <obo:RO_0001025 rdf:resource="http://purl.obolibrary.org/obo/GAZ_10000775"/>
        <obo:IAO_0000115>A stratovolcano that occupies an isolated location in the arid Danakil depression. It contains a large, central volcanotectonic depression that is open to the Zula Gulf and an isolated central cone. Jalua lies NW of basaltic lava flows of the Alid graben and south of the Zula Gulf.</obo:IAO_0000115>
        <oboInOwl:hasOBONamespace>GAZ</oboInOwl:hasOBONamespace>
        <oboInOwl:id>GAZ:00053598</oboInOwl:id>
        <rdfs:label>Jalua Volcano</rdfs:label>
    </owl:NamedIndividual>
    


    <!-- http://purl.obolibrary.org/obo/GAZ_00053599 -->

    <owl:NamedIndividual rdf:about="http://purl.obolibrary.org/obo/GAZ_00053599">
        <obo:RO_0001025 rdf:resource="http://purl.obolibrary.org/obo/GAZ_00051205"/>
        <obo:RO_0001025 rdf:resource="http://purl.obolibrary.org/obo/GAZ_10000775"/>
        <obo:IAO_0000115>An isolated, dissected stratovolcano in the central Danakil depression. The volcano is elongated in an E-W direction perpendicular to the orientation of the Alid graben. Alid consists of a structural dome of uplifted sedimentary rocks, capped by basaltic-to-rhyolitic lava flows, that rises 700 m above the graben floor.</obo:IAO_0000115>
        <oboInOwl:hasOBONamespace>GAZ</oboInOwl:hasOBONamespace>
        <oboInOwl:id>GAZ:00053599</oboInOwl:id>
        <rdfs:label>Alid Volcano</rdfs:label>
    </owl:NamedIndividual>
    


    <!-- http://purl.obolibrary.org/obo/GAZ_00053600 -->

    <owl:NamedIndividual rdf:about="http://purl.obolibrary.org/obo/GAZ_00053600">
        <obo:RO_0001025 rdf:resource="http://purl.obolibrary.org/obo/GAZ_00053602"/>
        <obo:IAO_0000115>Numerous phreatic explosion craters dot the Salt Plain NNE of the Erta Ale Range in one of the lowest areas of the desolate Danakil depression. These craters mark Earth&apos;s lowest known subaerial volcanic vents.</obo:IAO_0000115>
        <oboInOwl:hasOBONamespace>GAZ</oboInOwl:hasOBONamespace>
        <oboInOwl:id>GAZ:00053600</oboInOwl:id>
        <rdfs:label>Dallol Volcano</rdfs:label>
    </owl:NamedIndividual>
    


    <!-- http://purl.obolibrary.org/obo/GAZ_00053601 -->

    <owl:NamedIndividual rdf:about="http://purl.obolibrary.org/obo/GAZ_00053601">
        <obo:RO_0001025 rdf:resource="http://purl.obolibrary.org/obo/GAZ_00053602"/>
        <obo:IAO_0000115>A prominent stratovolcano at the northern end of the Erta Ale Range. It is formed of interstratified lava flows and hyaloclastites. Fumarolic activity is continuing, and a small lake filled by boiling mud occupies the crater.</obo:IAO_0000115>
        <oboInOwl:hasOBONamespace>GAZ</oboInOwl:hasOBONamespace>
        <oboInOwl:id>GAZ:00053601</oboInOwl:id>
        <rdfs:label>Gada Ale Volcano</rdfs:label>
    </owl:NamedIndividual>
    


    <!-- http://purl.obolibrary.org/obo/GAZ_00053602 -->

    <owl:NamedIndividual rdf:about="http://purl.obolibrary.org/obo/GAZ_00053602">
        <obo:RO_0001025 rdf:resource="http://purl.obolibrary.org/obo/GAZ_00051205"/>
        <obo:IAO_0000115>An axial volcanic chain of the Afar Region, Ethiopia. It consists mostly of shield volcanoes.</obo:IAO_0000115>
        <oboInOwl:hasOBONamespace>GAZ</oboInOwl:hasOBONamespace>
        <oboInOwl:id>GAZ:00053602</oboInOwl:id>
        <rdfs:label>Erta Ale Range</rdfs:label>
    </owl:NamedIndividual>
    


    <!-- http://purl.obolibrary.org/obo/GAZ_00053603 -->

    <owl:NamedIndividual rdf:about="http://purl.obolibrary.org/obo/GAZ_00053603">
        <obo:RO_0001025 rdf:resource="http://purl.obolibrary.org/obo/GAZ_00053602"/>
        <obo:IAO_0000115>An active shield volcano located in the Afar Region of northeastern Ethiopia. It is the most active volcano in Ethiopia. The broad, 50 km wide volcano rises more than 600 m from below sea level in the barren Danakil depression.</obo:IAO_0000115>
        <oboInOwl:hasOBONamespace>GAZ</oboInOwl:hasOBONamespace>
        <oboInOwl:id>GAZ:00053603</oboInOwl:id>
        <rdfs:label>Erta Ale Volcano</rdfs:label>
    </owl:NamedIndividual>
    


    <!-- http://purl.obolibrary.org/obo/GAZ_00053604 -->

    <owl:NamedIndividual rdf:about="http://purl.obolibrary.org/obo/GAZ_00053604">
        <obo:RO_0001025 rdf:resource="http://purl.obolibrary.org/obo/GAZ_00053602"/>
        <obo:IAO_0000115>An elongated, 1031 m high stratovolcano located SW of Erta Ale volcano. It is the highest of the Erta Ale Range volcanoes and is located west of the axis of the range. In contrast to other volcanoes of the Erta Ale Range, Ale Bagu is mantled by basaltic pyroclastic rocks. Summit craters are elongated along a NNW-SSE trend. The main crater is a steep-walled, 750 x 450 m depression occupied by a steep-sided lava cone that has fed trachytic lava flows over the crater floor.</obo:IAO_0000115>
        <oboInOwl:hasOBONamespace>GAZ</oboInOwl:hasOBONamespace>
        <oboInOwl:id>GAZ:00053604</oboInOwl:id>
        <rdfs:label>Ale Bagu Volcano</rdfs:label>
    </owl:NamedIndividual>
    


    <!-- http://purl.obolibrary.org/obo/GAZ_00053605 -->

    <owl:NamedIndividual rdf:about="http://purl.obolibrary.org/obo/GAZ_00053605">
        <obo:RO_0001025 rdf:resource="http://purl.obolibrary.org/obo/GAZ_00053602"/>
        <obo:IAO_0000115>A small, but steep-sided conical stratovolcano that rises 300 m above surrounding lava fields SE of Alu volcano. This morphology, unusual for the Erta Ale Range volcanoes, results from the extrusion of viscous, silicic lava flows with primary slopes up to about 35 degrees. These silicic flows extend primarily to the east; on the west they are blocked by walls of a horst structure along the crest of the Erta Ale range.</obo:IAO_0000115>
        <oboInOwl:hasOBONamespace>GAZ</oboInOwl:hasOBONamespace>
        <oboInOwl:id>GAZ:00053605</oboInOwl:id>
        <rdfs:label>Dalaffilla Volcano</rdfs:label>
    </owl:NamedIndividual>
    


    <!-- http://purl.obolibrary.org/obo/GAZ_00053606 -->

    <owl:NamedIndividual rdf:about="http://purl.obolibrary.org/obo/GAZ_00053606">
        <obo:RO_0001025 rdf:resource="http://purl.obolibrary.org/obo/GAZ_00053602"/>
        <obo:IAO_0000115>A system of volcanic fissures, located in Ethiopia. The fissures have produced silicic lava flows, and other fissures south of the volcano have formed huge youthful basaltic lava flows, which enlarge to the north as far as Lake Bakili. There is major fumarolic motion, which are located on frequent corresponding faults, some of which gave a lift up to 100 m.</obo:IAO_0000115>
        <oboInOwl:hasOBONamespace>GAZ</oboInOwl:hasOBONamespace>
        <oboInOwl:id>GAZ:00053606</oboInOwl:id>
        <rdfs:label>Alu Fissure Vents</rdfs:label>
    </owl:NamedIndividual>
    


    <!-- http://purl.obolibrary.org/obo/GAZ_00053607 -->

    <owl:NamedIndividual rdf:about="http://purl.obolibrary.org/obo/GAZ_00053607">
        <obo:RO_0001025 rdf:resource="http://purl.obolibrary.org/obo/GAZ_00053602"/>
        <obo:IAO_0000115>A complex stratovolcano located near the center of the Erta Ale Range. The earliest activity formed submarine lava flows partially covered by Quaternary reef deposits. An embryonic shield volcano is located on the SW side of the complex and is cut by curvilinear faults; youthful chains of spatter cones follow this same curvilinear pattern and form concentric semi-circles. The 668 m high summit of the Borale Ale complex is located on the NE side of the massif and consists of a silicic stratovolcano that is the largest of the Erte Ale Range. It has produced steep-sided viscous lava flows that have traveled up to 5 km from the volcano. Strong fumarolic activity occurs within a 300-m-wide summit crater.</obo:IAO_0000115>
        <oboInOwl:hasOBONamespace>GAZ</oboInOwl:hasOBONamespace>
        <oboInOwl:id>GAZ:00053607</oboInOwl:id>
        <rdfs:label>Borale Ale Volcano</rdfs:label>
    </owl:NamedIndividual>
    


    <!-- http://purl.obolibrary.org/obo/GAZ_00053608 -->

    <owl:NamedIndividual rdf:about="http://purl.obolibrary.org/obo/GAZ_00053608">
        <obo:RO_0001025 rdf:resource="http://purl.obolibrary.org/obo/GAZ_00053602"/>
        <obo:IAO_0000115>A shield volcano where tectonism has created a graben at the 521 m high summit. A symmetrical scoria cone with a 200-m-wide crater displaying fumarolic activity occupies the center of the graben. An older shield volcano is covered on the north by recent fissure-fed lava flows. Lava flows from the axial portion of a fissure system extending to the south have reached the floor of the Giulietti Plain south of the Erta Ale Range. The open fissures extend for more than 10 km and are lined with dozens of small spatter cones and pit craters.</obo:IAO_0000115>
        <oboInOwl:hasOBONamespace>GAZ</oboInOwl:hasOBONamespace>
        <oboInOwl:id>GAZ:00053608</oboInOwl:id>
        <rdfs:label>Hayli Gubbi Volcano</rdfs:label>
    </owl:NamedIndividual>
    


    <!-- http://purl.obolibrary.org/obo/GAZ_00053609 -->

    <owl:NamedIndividual rdf:about="http://purl.obolibrary.org/obo/GAZ_00053609">
        <obo:RO_0001025 rdf:resource="http://purl.obolibrary.org/obo/GAZ_00051205"/>
        <obo:RO_0001025 rdf:resource="http://purl.obolibrary.org/obo/GAZ_10000775"/>
        <obo:IAO_0000115>A stratovolcano located east of the Erta Ale Range and south of the crystalline basement rocks of the Danakil Alps. It is a large volcanic massif that rises to 1625 m above the western shore of the Red Sea. About 20 small cinder cones are located at the summit, and extensive basaltic lava fields to the north and NE, known as the Edd lava field, cover an area of 2700 km2 and reach the Red Sea coast.</obo:IAO_0000115>
        <oboInOwl:hasOBONamespace>GAZ</oboInOwl:hasOBONamespace>
        <oboInOwl:id>GAZ:00053609</oboInOwl:id>
        <rdfs:label>Dubbi Volcano</rdfs:label>
    </owl:NamedIndividual>
    


    <!-- http://purl.obolibrary.org/obo/GAZ_00053610 -->

    <owl:NamedIndividual rdf:about="http://purl.obolibrary.org/obo/GAZ_00053610">
        <obo:RO_0001025 rdf:resource="http://purl.obolibrary.org/obo/GAZ_00051205"/>
        <obo:RO_0001025 rdf:resource="http://purl.obolibrary.org/obo/GAZ_10000775"/>
        <obo:IAO_0000115>A stratovolcano in the Danakil depression of northern Ethiopia and Eritrea. Located at the SE end of the Danakil Alps, Nabro lies in the Danakil horst. Nabro is the most prominent and NE-most of three volcanoes with large summit calderas aligned in a NE-SW direction SW of Dubbi volcano. These three volcanoes, along with Sork Ale volcano, collectively comprise the Bidu volcanic complex. The complex Nabro stratovolcano is truncated by nested calderas, 8 and 5 km in diameter. The larger caldera is widely breached to the SW. Nabro was constructed primarily of trachytic lava flows and pyroclastics. Post-caldera rhyolitic obsidian domes and basaltic lava flows were erupted inside the caldera and on its flanks.</obo:IAO_0000115>
        <oboInOwl:hasOBONamespace>GAZ</oboInOwl:hasOBONamespace>
        <oboInOwl:id>GAZ:00053610</oboInOwl:id>
        <rdfs:label>Nabro Volcano</rdfs:label>
    </owl:NamedIndividual>
    


    <!-- http://purl.obolibrary.org/obo/GAZ_00053611 -->

    <owl:NamedIndividual rdf:about="http://purl.obolibrary.org/obo/GAZ_00053611">
        <obo:RO_0001025 rdf:resource="http://purl.obolibrary.org/obo/GAZ_00000581"/>
        <oboInOwl:hasOBONamespace>GAZ</oboInOwl:hasOBONamespace>
        <oboInOwl:id>GAZ:00053611</oboInOwl:id>
        <rdfs:label>Bidu Volcanic Complex</rdfs:label>
    </owl:NamedIndividual>
    


    <!-- http://purl.obolibrary.org/obo/GAZ_00053612 -->

    <owl:NamedIndividual rdf:about="http://purl.obolibrary.org/obo/GAZ_00053612">
        <obo:RO_0001025 rdf:resource="http://purl.obolibrary.org/obo/GAZ_00053611"/>
        <obo:IAO_0000115>A silicic stratovolcano located in the Danakil horst SE of Mallahle volcano. Sork Ale was constructed perpendicular to the NE-SW orientation of three larger stratovolcanoes of the Nabro volcanic range at the southern end of the Danakil Alps. A small, roughly 1 km wide, 300-m-deep steep-walled caldera is found at the summit of the 1611 m high volcano. Basaltic lava flows are prominent on the eastern side of the volcano, and satellite vents are located on the SE flank.</obo:IAO_0000115>
        <oboInOwl:hasOBONamespace>GAZ</oboInOwl:hasOBONamespace>
        <oboInOwl:id>GAZ:00053612</oboInOwl:id>
        <rdfs:label>Sork&apos;Ale Volcano</rdfs:label>
    </owl:NamedIndividual>
    


    <!-- http://purl.obolibrary.org/obo/GAZ_00053613 -->

    <owl:NamedIndividual rdf:about="http://purl.obolibrary.org/obo/GAZ_00053613">
        <obo:RO_0001025 rdf:resource="http://purl.obolibrary.org/obo/GAZ_00053611"/>
        <oboInOwl:hasOBONamespace>GAZ</oboInOwl:hasOBONamespace>
        <oboInOwl:id>GAZ:00053613</oboInOwl:id>
        <rdfs:label>Bara Ale Volcano</rdfs:label>
    </owl:NamedIndividual>
    


    <!-- http://purl.obolibrary.org/obo/GAZ_00053614 -->

    <owl:NamedIndividual rdf:about="http://purl.obolibrary.org/obo/GAZ_00053614">
        <obo:RO_0001025 rdf:resource="http://purl.obolibrary.org/obo/GAZ_00053611"/>
        <obo:IAO_0000115>A stratovolcano in the Danakil horst SW of Dubbi volcano, and lies SSW of Nabro volcano. These two volcanoes, along with Bara Ale and Sork&apos;Ale, form the Bidu volcanic complex. The complex Mallahle stratovolcano is truncated by a steep-walled 6 km wide caldera. Mallahle is formed of rhyolitic lava flows and pyroclastics. Basaltic lava flows blanket the slopes of the volcano.</obo:IAO_0000115>
        <oboInOwl:hasOBONamespace>GAZ</oboInOwl:hasOBONamespace>
        <oboInOwl:id>GAZ:00053614</oboInOwl:id>
        <rdfs:label>Mallahle Volcano</rdfs:label>
    </owl:NamedIndividual>
    


    <!-- http://purl.obolibrary.org/obo/GAZ_00053619 -->

    <owl:NamedIndividual rdf:about="http://purl.obolibrary.org/obo/GAZ_00053619">
        <obo:RO_0001025 rdf:resource="http://purl.obolibrary.org/obo/GAZ_00051205"/>
        <obo:IAO_0000115>A saline lake in northern Ethiopia. Located in the Administrative Zone 2, it is one of the lakes of the Afar Depression.</obo:IAO_0000115>
        <oboInOwl:hasOBONamespace>GAZ</oboInOwl:hasOBONamespace>
        <oboInOwl:id>GAZ:00053619</oboInOwl:id>
        <rdfs:label>Lake Afrera</rdfs:label>
    </owl:NamedIndividual>
    


    <!-- http://purl.obolibrary.org/obo/GAZ_00053620 -->

    <owl:NamedIndividual rdf:about="http://purl.obolibrary.org/obo/GAZ_00053620">
        <obo:RO_0001025 rdf:resource="http://purl.obolibrary.org/obo/GAZ_00053632"/>
        <obo:IAO_0000115>A stratovolcano that rises above the eastern shore of Lake Afrera, also known as Lake Giulietti. The upper part of the 812 m high conical volcano consists of trachytic lava flows overlying older basaltic flows. Young pantelleritic obsidian domes south of the volcano are the probable source of rounded pumice fragments found around Lake Afrera.</obo:IAO_0000115>
        <oboInOwl:hasOBONamespace>GAZ</oboInOwl:hasOBONamespace>
        <oboInOwl:id>GAZ:00053620</oboInOwl:id>
        <rdfs:label>Borawli Volcano</rdfs:label>
    </owl:NamedIndividual>
    


    <!-- http://purl.obolibrary.org/obo/GAZ_00053622 -->

    <owl:NamedIndividual rdf:about="http://purl.obolibrary.org/obo/GAZ_00053622">
        <obo:RO_0001025 rdf:resource="http://purl.obolibrary.org/obo/GAZ_00051205"/>
        <obo:IAO_0000115>An 1815 m high stratovolcano located well to the west of the Danakil depression at the foot of the regional Ethiopian scarp. The volcano is situated between two large horsts of uplifted basement blocks. A large trachytic and rhyolitic stratovolcano at the center of the Ma Alalta complex contains nested oval-shaped summit calderas, 8 x 5 km and 5 x 2.5 km wide. Ignimbrite deposits, perhaps associated with formation of the larger caldera, extend beyond the volcano primarily to the NE and SE. Young basaltic lava flows were erupted on the NW, SE, and eastern flanks of the volcano. Recent silicic activity has produced pantelleritic obsidian domes and lava flows on the volcano&apos;s southern flank. Fumarolic activity continues at one of the domes.</obo:IAO_0000115>
        <oboInOwl:hasOBONamespace>GAZ</oboInOwl:hasOBONamespace>
        <oboInOwl:id>GAZ:00053622</oboInOwl:id>
        <rdfs:label>Ma Alalta Volcano</rdfs:label>
    </owl:NamedIndividual>
    


    <!-- http://purl.obolibrary.org/obo/GAZ_00053623 -->

    <owl:NamedIndividual rdf:about="http://purl.obolibrary.org/obo/GAZ_00053623">
        <obo:RO_0001025 rdf:resource="http://purl.obolibrary.org/obo/GAZ_00051205"/>
        <obo:IAO_0000115>A shield volcano covers an area of 2700 km2 in the western Danakil depression SW of Lake Afrera. A series of very recent craters is aligned along the NNW-trending axis of the basaltic-to-trachytic shield. The Alayta lava field, covered by very fresh lava flows, was erupted from N-S-trending fissures along the east side of the shield volcano and laps up against the western flank of Afdera volcano.</obo:IAO_0000115>
        <oboInOwl:hasOBONamespace>GAZ</oboInOwl:hasOBONamespace>
        <oboInOwl:id>GAZ:00053623</oboInOwl:id>
        <rdfs:label>Alayta Volcano</rdfs:label>
    </owl:NamedIndividual>
    


    <!-- http://purl.obolibrary.org/obo/GAZ_00053624 -->

    <owl:NamedIndividual rdf:about="http://purl.obolibrary.org/obo/GAZ_00053624">
        <obo:RO_0001025 rdf:resource="http://purl.obolibrary.org/obo/GAZ_00051205"/>
        <obo:IAO_0000115>A Holocene stratovolcanic massif forming an axial range of the Afar depression SSW of the Alayta massif. Pantelleritic obsidian flows, lava domes, and pumice cones form the summit and upper flanks of the volcano, which rises above the Teru Plain and was built over a base of basaltic-to-trachytic lava flows of a shield volcano. Late-stage basaltic fissure eruptions occurred at the NW base of the volcano. Abundant fumaroles are located along the crest of the volcano and extend NE towards Alayta volcano.</obo:IAO_0000115>
        <oboInOwl:hasOBONamespace>GAZ</oboInOwl:hasOBONamespace>
        <oboInOwl:id>GAZ:00053624</oboInOwl:id>
        <rdfs:label>Dabbahu Volcano</rdfs:label>
    </owl:NamedIndividual>
    


    <!-- http://purl.obolibrary.org/obo/GAZ_00053625 -->

    <owl:NamedIndividual rdf:about="http://purl.obolibrary.org/obo/GAZ_00053625">
        <obo:RO_0001025 rdf:resource="http://purl.obolibrary.org/obo/GAZ_00051205"/>
        <obo:IAO_0000115>A shield volcano that was constructed along an offshoot of the Ethiopian escarpment, SW of the Teru plain. In contrast to structural trends in other parts of Afar, Dabbayra consists of a basaltic shield volcano elongated in an ENE-WSW direction. The only silicic volcanic rocks are a NNW-trending line of lava domes and lava flows near the crest of the 1302 m high volcano.</obo:IAO_0000115>
        <oboInOwl:hasOBONamespace>GAZ</oboInOwl:hasOBONamespace>
        <oboInOwl:id>GAZ:00053625</oboInOwl:id>
        <rdfs:label>Dabbayra Volcano</rdfs:label>
    </owl:NamedIndividual>
    


    <!-- http://purl.obolibrary.org/obo/GAZ_00053626 -->

    <owl:NamedIndividual rdf:about="http://purl.obolibrary.org/obo/GAZ_00053626">
        <obo:RO_0001025 rdf:resource="http://purl.obolibrary.org/obo/GAZ_00051205"/>
        <obo:IAO_0000115>A complex of shield volcanoes located in the Kalo plain, SSE of Dabbahu volcano. The massive complex is 105 km long and 20-30 km wide, and represents an uplifted segment of a mid-ocean ridge spreading center. A small basaltic shield volcano is located at the northern end of the complex, south of which is an area of abundant fissure-fed lava flows. Two basaltic shield volcanoes, the largest of which is Unda Hararo, occupy the center of the complex. The dominant part of the complex lies to the south, where the Gumatmali-Gablaytu fissure system is located. Voluminous fluid lava flows issued from these NNW-trending fissures, and solidified lava lakes occupy two large craters. The small Gablaytu shield volcano forms the SE-most end of the Manda Hararo complex. Lava flows from Gablaytu and from Manda overlie 8000-year-old sediments. Hot springs and fumaroles occur around Daorre lake.</obo:IAO_0000115>
        <oboInOwl:hasOBONamespace>GAZ</oboInOwl:hasOBONamespace>
        <oboInOwl:id>GAZ:00053626</oboInOwl:id>
        <rdfs:label>Manda Hararo Volcanic Complex</rdfs:label>
    </owl:NamedIndividual>
    


    <!-- http://purl.obolibrary.org/obo/GAZ_00053627 -->

    <owl:NamedIndividual rdf:about="http://purl.obolibrary.org/obo/GAZ_00053627">
        <obo:RO_0001025 rdf:resource="http://purl.obolibrary.org/obo/GAZ_00053626"/>
        <obo:IAO_0000115>A shield volcano.</obo:IAO_0000115>
        <oboInOwl:hasOBONamespace>GAZ</oboInOwl:hasOBONamespace>
        <oboInOwl:id>GAZ:00053627</oboInOwl:id>
        <rdfs:label>Gablaytu Volcano</rdfs:label>
    </owl:NamedIndividual>
    


    <!-- http://purl.obolibrary.org/obo/GAZ_00053628 -->

    <owl:NamedIndividual rdf:about="http://purl.obolibrary.org/obo/GAZ_00053628">
        <obo:RO_0001025 rdf:resource="http://purl.obolibrary.org/obo/GAZ_00053626"/>
        <obo:IAO_0000115>A fissure system.</obo:IAO_0000115>
        <oboInOwl:hasOBONamespace>GAZ</oboInOwl:hasOBONamespace>
        <oboInOwl:id>GAZ:00053628</oboInOwl:id>
        <rdfs:label>Gumatmali-Gablaytu Fissure System</rdfs:label>
    </owl:NamedIndividual>
    


    <!-- http://purl.obolibrary.org/obo/GAZ_00053629 -->

    <owl:NamedIndividual rdf:about="http://purl.obolibrary.org/obo/GAZ_00053629">
        <obo:RO_0001025 rdf:resource="http://purl.obolibrary.org/obo/GAZ_00053626"/>
        <obo:IAO_0000115>A basaltic shield volcano.</obo:IAO_0000115>
        <oboInOwl:hasOBONamespace>GAZ</oboInOwl:hasOBONamespace>
        <oboInOwl:id>GAZ:00053629</oboInOwl:id>
        <rdfs:label>Unda Hararo Volcano</rdfs:label>
    </owl:NamedIndividual>
    


    <!-- http://purl.obolibrary.org/obo/GAZ_00053630 -->

    <owl:NamedIndividual rdf:about="http://purl.obolibrary.org/obo/GAZ_00053630">
        <obo:RO_0001025 rdf:resource="http://purl.obolibrary.org/obo/GAZ_00051205"/>
        <obo:IAO_0000115>A small 930 m high alkali rhyolitic stratovolcano located in the western Afar near the Ethiopian escarpment, NE of Dessye.</obo:IAO_0000115>
        <oboInOwl:hasOBONamespace>GAZ</oboInOwl:hasOBONamespace>
        <oboInOwl:id>GAZ:00053630</oboInOwl:id>
        <rdfs:label>Groppo Volcano</rdfs:label>
    </owl:NamedIndividual>
    


    <!-- http://purl.obolibrary.org/obo/GAZ_00053631 -->

    <owl:NamedIndividual rdf:about="http://purl.obolibrary.org/obo/GAZ_00053631">
        <obo:RO_0001025 rdf:resource="http://purl.obolibrary.org/obo/GAZ_00051205"/>
        <obo:IAO_0000115>A shield volcano that lies in the Saha Plain, SE of the Manda Hararo complex in the South Danakil region. Wind-blown sand fills the summit crater of the young basaltic volcano. Initial subaqueous activity occurred along NNW-trending fissures. Fumarolic activity observed in the 1930s was not seen during field work in the 1970s.</obo:IAO_0000115>
        <oboInOwl:hasOBONamespace>GAZ</oboInOwl:hasOBONamespace>
        <oboInOwl:id>GAZ:00053631</oboInOwl:id>
        <rdfs:label>Kurub Volcano</rdfs:label>
    </owl:NamedIndividual>
    


    <!-- http://purl.obolibrary.org/obo/GAZ_00053632 -->

    <owl:NamedIndividual rdf:about="http://purl.obolibrary.org/obo/GAZ_00053632">
        <obo:RO_0001025 rdf:resource="http://purl.obolibrary.org/obo/GAZ_00051205"/>
        <obo:IAO_0000115>A group of rhyolitic lava domes on the floor of the southern Kali plain, north of Aysa&apos;iyta.</obo:IAO_0000115>
        <oboInOwl:hasOBONamespace>GAZ</oboInOwl:hasOBONamespace>
        <oboInOwl:id>GAZ:00053632</oboInOwl:id>
        <rdfs:label>Borawli Volcanic Complex</rdfs:label>
    </owl:NamedIndividual>
    


    <!-- http://purl.obolibrary.org/obo/GAZ_00053635 -->

    <owl:NamedIndividual rdf:about="http://purl.obolibrary.org/obo/GAZ_00053635">
        <rdf:type rdf:resource="http://purl.obolibrary.org/obo/ENVO_00000354"/>
        <obo:IAO_0000115>A volcanic complex that is a large Holocene stratovolcano constructed along the border between Ethiopia, Eritrea, and Djibouti. The 2028 m high trachytic-to-rhyolitic volcano is the most prominent topographic feature in this area and towers above its neighbor to the SW, Manda Inakir. Rhyolitic lava domes and lava flows are found in the summit region, which is truncated by a caldera.</obo:IAO_0000115>
        <oboInOwl:hasOBONamespace>GAZ</oboInOwl:hasOBONamespace>
        <oboInOwl:id>GAZ:00053635</oboInOwl:id>
        <rdfs:label>Mousa Alli Volcanic Complex</rdfs:label>
    </owl:NamedIndividual>
    


    <!-- http://purl.obolibrary.org/obo/GAZ_00053636 -->

    <owl:NamedIndividual rdf:about="http://purl.obolibrary.org/obo/GAZ_00053636">
        <obo:RO_0001025 rdf:resource="http://purl.obolibrary.org/obo/GAZ_00000777"/>
        <obo:IAO_0000115>A volcanic field, located along the Eritrea/Djibouti border, consists of a group of basaltic scoria cones and lava flows aligned in an E-W direction NE of the large Mousa Alli stratovolcano. A second E-W-trending chain of cones is located to the north of the principal chain, most of which lies in Eritrea, and fed long lava flows that descend to the north, in the direction of the Red Sea.</obo:IAO_0000115>
        <oboInOwl:hasOBONamespace>GAZ</oboInOwl:hasOBONamespace>
        <oboInOwl:id>GAZ:00053636</oboInOwl:id>
        <rdfs:label>Gufa Volcanic Field</rdfs:label>
    </owl:NamedIndividual>
    


    <!-- http://purl.obolibrary.org/obo/GAZ_00053637 -->

    <owl:NamedIndividual rdf:about="http://purl.obolibrary.org/obo/GAZ_00053637">
        <obo:RO_0001025 rdf:resource="http://purl.obolibrary.org/obo/GAZ_00000777"/>
        <obo:IAO_0000115>A volcanic field near the Red Sea coast in southern Eritrea forms a spectacular range of basaltic cinder cones and associated lava flows. The massive lava field covers a 55 x 90 km area, and flows reached the Red Sea along a broad front. The vents of the Assab volcanic field were constructed along a broad E-W-trending line that extends to the coastal city of Assab.</obo:IAO_0000115>
        <oboInOwl:hasOBONamespace>GAZ</oboInOwl:hasOBONamespace>
        <oboInOwl:id>GAZ:00053637</oboInOwl:id>
        <rdfs:label>Assab Volcanic Field</rdfs:label>
    </owl:NamedIndividual>
    


    <!-- http://purl.obolibrary.org/obo/GAZ_00053663 -->

    <owl:NamedIndividual rdf:about="http://purl.obolibrary.org/obo/GAZ_00053663">
        <obo:RO_0001025 rdf:resource="http://purl.obolibrary.org/obo/GAZ_00000007"/>
        <obo:IAO_0000115>A freshwater lake in the Oromia Region of Ethiopia, about 100 km south of the capital, Addis Ababa, on the border between the Misraq Shewa and Arsi Zones. It is located in the Great Rift Valley at an elevation of 1,585 meters to the east of Lake Abijatta.</obo:IAO_0000115>
        <oboInOwl:hasOBONamespace>GAZ</oboInOwl:hasOBONamespace>
        <oboInOwl:id>GAZ:00053663</oboInOwl:id>
        <rdfs:label>Lake Langano</rdfs:label>
    </owl:NamedIndividual>
    


    <!-- http://purl.obolibrary.org/obo/GAZ_00053667 -->

    <owl:NamedIndividual rdf:about="http://purl.obolibrary.org/obo/GAZ_00053667">
        <obo:RO_0001025 rdf:resource="http://purl.obolibrary.org/obo/GAZ_00000007"/>
        <obo:IAO_0000115>A lake that is surrounded by hot springs filled with boiling water, and the earth surrounding the lake is filled with cracks due to erosion and earthquakes. Due to steam rising from the boiling water in the springs, the atmosphere around the lake is relatively foggy.</obo:IAO_0000115>
        <oboInOwl:hasOBONamespace>GAZ</oboInOwl:hasOBONamespace>
        <oboInOwl:id>GAZ:00053667</oboInOwl:id>
        <rdfs:label>Lake Shala</rdfs:label>
    </owl:NamedIndividual>
    


    <!-- http://purl.obolibrary.org/obo/GAZ_00053668 -->

    <owl:NamedIndividual rdf:about="http://purl.obolibrary.org/obo/GAZ_00053668">
        <obo:RO_0001025 rdf:resource="http://purl.obolibrary.org/obo/GAZ_00053667"/>
        <obo:IAO_0000115>An island in Lake Shala.</obo:IAO_0000115>
        <oboInOwl:hasOBONamespace>GAZ</oboInOwl:hasOBONamespace>
        <oboInOwl:id>GAZ:00053668</oboInOwl:id>
        <rdfs:label>Pelican Island</rdfs:label>
    </owl:NamedIndividual>
    


    <!-- http://purl.obolibrary.org/obo/GAZ_00053675 -->

    <owl:NamedIndividual rdf:about="http://purl.obolibrary.org/obo/GAZ_00053675">
        <obo:RO_0001025 rdf:resource="http://purl.obolibrary.org/obo/GAZ_00000007"/>
        <obo:IAO_0000115>A lake in the Southern Nations, Nationalities, and Peoples Region of southern Ethiopia. It is located in the Great Rift Valley at an elevation of 1,235 meters. It is just to the south of Lake Abaya and the city of Arba Minch, and east of the Guge Mountains. Lake Chamo does not always have an outflow, but in some years, it overflows into the Sagan River. In some years, it is fed by overflow from Lake Abaya.</obo:IAO_0000115>
        <oboInOwl:hasOBONamespace>GAZ</oboInOwl:hasOBONamespace>
        <oboInOwl:id>GAZ:00053675</oboInOwl:id>
        <rdfs:label>Lake Chamo</rdfs:label>
    </owl:NamedIndividual>
    


    <!-- http://purl.obolibrary.org/obo/GAZ_00053679 -->

    <owl:NamedIndividual rdf:about="http://purl.obolibrary.org/obo/GAZ_00053679">
        <obo:RO_0001025 rdf:resource="http://purl.obolibrary.org/obo/GAZ_00051205"/>
        <obo:IAO_0000115>A vegetated rhyolitic stratovolcano, located south of the Asbahri plain in the southern Afar region. On its eastern side, 2145 m high Ayelu is cut by regional faults and is overlain by ignimbrites erupted from Adwa volcano immediately to the east. Ayelu was constructed by a series of thick rhyolitic lava flows, creating a higher and steeper-sided volcano than its neighbor Adwa. Hot springs are located on the western flank of Ayelu.</obo:IAO_0000115>
        <oboInOwl:hasOBONamespace>GAZ</oboInOwl:hasOBONamespace>
        <oboInOwl:id>GAZ:00053679</oboInOwl:id>
        <rdfs:label>Mount Ayalu</rdfs:label>
    </owl:NamedIndividual>
    


    <!-- http://purl.obolibrary.org/obo/GAZ_00057510 -->

    <owl:NamedIndividual rdf:about="http://purl.obolibrary.org/obo/GAZ_00057510">
        <obo:RO_0001025 rdf:resource="http://purl.obolibrary.org/obo/GAZ_00051205"/>
        <obo:IAO_0000115>An endorheic saline lake lying on the Ethiopia-Djibouti border, and is one of a chain of six connected lakes which also includes (from north to south) lakes Gargori, Laitali, Gummare, Bario and Afambo. Lake Abbe is the ultimate destination of the waters of the Awash River. Lake Abbe is at the central point of the Afar Depression, where three pieces of the earth&apos;s crust meet. On the northwest shore rises Dama Ali, a volcanic mountain.</obo:IAO_0000115>
        <oboInOwl:hasOBONamespace>GAZ</oboInOwl:hasOBONamespace>
        <oboInOwl:id>GAZ:00057510</oboInOwl:id>
        <rdfs:label>Lake Abbe</rdfs:label>
    </owl:NamedIndividual>
    


    <!-- http://purl.obolibrary.org/obo/GAZ_00057758 -->

    <owl:NamedIndividual rdf:about="http://purl.obolibrary.org/obo/GAZ_00057758">
        <obo:RO_0001025 rdf:resource="http://purl.obolibrary.org/obo/GAZ_00000777"/>
        <obo:IAO_0000115>A desert located in north eastern Ethiopia and in southern Eritrea, where it forms the Southern Red Sea district.</obo:IAO_0000115>
        <oboInOwl:hasOBONamespace>GAZ</oboInOwl:hasOBONamespace>
        <oboInOwl:id>GAZ:00057758</oboInOwl:id>
        <rdfs:label>Danakil Desert</rdfs:label>
    </owl:NamedIndividual>
    


    <!-- http://purl.obolibrary.org/obo/GAZ_00058384 -->

    <owl:NamedIndividual rdf:about="http://purl.obolibrary.org/obo/GAZ_00058384">
        <obo:RO_0001025 rdf:resource="http://purl.obolibrary.org/obo/GAZ_00008742"/>
        <obo:IAO_0000115>A lake that was drained in the 1950s, but is now being regenerated.</obo:IAO_0000115>
        <oboInOwl:hasOBONamespace>GAZ</oboInOwl:hasOBONamespace>
        <oboInOwl:id>GAZ:00058384</oboInOwl:id>
        <rdfs:label>Lake Hulah</rdfs:label>
    </owl:NamedIndividual>
    


    <!-- http://purl.obolibrary.org/obo/GAZ_00058395 -->

    <owl:NamedIndividual rdf:about="http://purl.obolibrary.org/obo/GAZ_00058395">
        <obo:RO_0001025 rdf:resource="http://purl.obolibrary.org/obo/GAZ_00058396"/>
        <obo:IAO_0000115>An artificial lake located in the southern region of the Beqaa Valley. Made by damming the Litani River.</obo:IAO_0000115>
        <oboInOwl:hasOBONamespace>GAZ</oboInOwl:hasOBONamespace>
        <oboInOwl:id>GAZ:00058395</oboInOwl:id>
        <rdfs:label>Lake Qaraoun</rdfs:label>
    </owl:NamedIndividual>
    


    <!-- http://purl.obolibrary.org/obo/GAZ_00058396 -->

    <owl:NamedIndividual rdf:about="http://purl.obolibrary.org/obo/GAZ_00058396">
        <obo:RO_0001025 rdf:resource="http://purl.obolibrary.org/obo/GAZ_00044906"/>
        <obo:IAO_0000115>A river that rises west of Baalbek in the fertile Beqaa Valley and empties in the Mediterranean Sea north of Tyre.</obo:IAO_0000115>
        <oboInOwl:hasOBONamespace>GAZ</oboInOwl:hasOBONamespace>
        <oboInOwl:id>GAZ:00058396</oboInOwl:id>
        <rdfs:label>Litani River</rdfs:label>
    </owl:NamedIndividual>
    


    <!-- http://purl.obolibrary.org/obo/GAZ_00058780 -->

    <owl:NamedIndividual rdf:about="http://purl.obolibrary.org/obo/GAZ_00058780">
        <obo:RO_0001025 rdf:resource="http://purl.obolibrary.org/obo/GAZ_00058782"/>
        <obo:IAO_0000115>A lake lagoon in Zambia. It is the largest of several lagoons in the Luapula River swamps south of Lake Mweru, in the Luapula Province of Zambia.</obo:IAO_0000115>
        <oboInOwl:hasOBONamespace>GAZ</oboInOwl:hasOBONamespace>
        <oboInOwl:id>GAZ:00058780</oboInOwl:id>
        <rdfs:label>Mofwe Lagoon</rdfs:label>
    </owl:NamedIndividual>
    


    <!-- http://purl.obolibrary.org/obo/GAZ_00058781 -->

    <owl:NamedIndividual rdf:about="http://purl.obolibrary.org/obo/GAZ_00058781">
        <obo:IAO_0000115>A river that drains the northern Zambian plateau north of Kawambwa and flows west into the Luapula valley. It enters the Luapula swamps near the Mofwe Lagoon.</obo:IAO_0000115>
        <oboInOwl:hasOBONamespace>GAZ</oboInOwl:hasOBONamespace>
        <oboInOwl:id>GAZ:00058781</oboInOwl:id>
        <rdfs:label>Mbereshi River</rdfs:label>
    </owl:NamedIndividual>
    


    <!-- http://purl.obolibrary.org/obo/GAZ_00058782 -->

    <owl:NamedIndividual rdf:about="http://purl.obolibrary.org/obo/GAZ_00058782">
        <obo:IAO_0000115>Swamps that stretch along the last 100 km of the Luapula River before it reaches the Lake Mweru, and for much of that they are 30 km wide, covering and area of about 2500 km2. There are four inhabited islands in the DR Congo part of the delta, including the largest in the system which is connected to dry land in the dry season. Zambia has three inhabited islands in the delta including Chisenga Island. The are also many lagoons, the largest of which is Mofwe Lagoon on the Zambian side.</obo:IAO_0000115>
        <oboInOwl:hasOBONamespace>GAZ</oboInOwl:hasOBONamespace>
        <oboInOwl:id>GAZ:00058782</oboInOwl:id>
        <rdfs:label>Luapula Swamps</rdfs:label>
    </owl:NamedIndividual>
    


    <!-- http://purl.obolibrary.org/obo/GAZ_00058783 -->

    <owl:NamedIndividual rdf:about="http://purl.obolibrary.org/obo/GAZ_00058783">
        <obo:RO_0001025 rdf:resource="http://purl.obolibrary.org/obo/GAZ_00058782"/>
        <obo:IAO_0000115>A Zambian island in the Luapula Swamps.</obo:IAO_0000115>
        <oboInOwl:hasOBONamespace>GAZ</oboInOwl:hasOBONamespace>
        <oboInOwl:id>GAZ:00058783</oboInOwl:id>
        <rdfs:label>Chisenga Island</rdfs:label>
    </owl:NamedIndividual>
    


    <!-- http://purl.obolibrary.org/obo/GAZ_00058791 -->

    <owl:NamedIndividual rdf:about="http://purl.obolibrary.org/obo/GAZ_00058791">
        <obo:RO_0001025 rdf:resource="http://purl.obolibrary.org/obo/GAZ_00000007"/>
        <obo:IAO_0000115>A polymictic shallow lake complex of Uganda, about 1,720 km2 in area and at an elevation of 914 m. The Victoria Nile flows through the lake on its way from Lake Victoria to Lake Albert. The main inflow from Lake Victoria is regulated by the Nalubaale Power Station in Jinja. Another source of water is the Mount Elgon region on the border between Uganda and Kenya.</obo:IAO_0000115>
        <oboInOwl:hasOBONamespace>GAZ</oboInOwl:hasOBONamespace>
        <oboInOwl:id>GAZ:00058791</oboInOwl:id>
        <rdfs:label>Lake Kyoga</rdfs:label>
    </owl:NamedIndividual>
    


    <!-- http://purl.obolibrary.org/obo/GAZ_00058792 -->

    <owl:NamedIndividual rdf:about="http://purl.obolibrary.org/obo/GAZ_00058792">
        <obo:RO_0001025 rdf:resource="http://purl.obolibrary.org/obo/GAZ_00000007"/>
        <obo:IAO_0000115>A lake in Uganda. It drains to the SW into Lake Edward through the Kazinga Channel.</obo:IAO_0000115>
        <oboInOwl:hasOBONamespace>GAZ</oboInOwl:hasOBONamespace>
        <oboInOwl:id>GAZ:00058792</oboInOwl:id>
        <rdfs:label>Lake George</rdfs:label>
    </owl:NamedIndividual>
    


    <!-- http://purl.obolibrary.org/obo/GAZ_00058802 -->

    <owl:NamedIndividual rdf:about="http://purl.obolibrary.org/obo/GAZ_00058802">
        <obo:RO_0001025 rdf:resource="http://purl.obolibrary.org/obo/GAZ_00000007"/>
        <obo:RO_0001025 rdf:resource="http://purl.obolibrary.org/obo/GAZ_00136138"/>
        <obo:IAO_0000115>The world&apos;s largest unbroken, unflooded volcanic caldera. The Crater, which formed when a giant volcano exploded and collapsed on itself some two to three million years ago, is 610m deep and the floor is 260 km2.</obo:IAO_0000115>
        <oboInOwl:hasOBONamespace>GAZ</oboInOwl:hasOBONamespace>
        <oboInOwl:id>GAZ:00058802</oboInOwl:id>
        <rdfs:label>Ngorongoro Crater</rdfs:label>
    </owl:NamedIndividual>
    


    <!-- http://purl.obolibrary.org/obo/GAZ_00058803 -->

    <owl:NamedIndividual rdf:about="http://purl.obolibrary.org/obo/GAZ_00058803">
        <obo:RO_0001025 rdf:resource="http://purl.obolibrary.org/obo/GAZ_00000007"/>
        <obo:IAO_0000115>A steep-sided ravine in the Great Rift Valley, which stretches along eastern Africa. Olduvai is in the eastern Serengeti Plains in northern Tanzania and is about 30 miles long.</obo:IAO_0000115>
        <oboInOwl:hasOBONamespace>GAZ</oboInOwl:hasOBONamespace>
        <oboInOwl:id>GAZ:00058803</oboInOwl:id>
        <rdfs:label>Olduvai Gorge</rdfs:label>
    </owl:NamedIndividual>
    


    <!-- http://purl.obolibrary.org/obo/GAZ_00058835 -->

    <owl:NamedIndividual rdf:about="http://purl.obolibrary.org/obo/GAZ_00058835">
        <obo:RO_0001025 rdf:resource="http://purl.obolibrary.org/obo/GAZ_00058836"/>
        <obo:IAO_0000115>An oxbow lake in Kenya, at the base of the Kerio valley. The lake is 1 km2 in size. It was formed in year 1961 as a result of the Kerio River changing its course, therefore forming an oxbow lake.</obo:IAO_0000115>
        <oboInOwl:hasOBONamespace>GAZ</oboInOwl:hasOBONamespace>
        <oboInOwl:id>GAZ:00058835</oboInOwl:id>
        <rdfs:label>Lake Kamnarok</rdfs:label>
    </owl:NamedIndividual>
    


    <!-- http://purl.obolibrary.org/obo/GAZ_00058836 -->

    <owl:NamedIndividual rdf:about="http://purl.obolibrary.org/obo/GAZ_00058836">
        <obo:RO_0001025 rdf:resource="http://purl.obolibrary.org/obo/GAZ_00000007"/>
        <obo:IAO_0000115>A valley that lies between the Tugen Hills and the Elgeyo escarpment at an elevation of 1,000 m. in the Great Rift Valley in Kenya.</obo:IAO_0000115>
        <oboInOwl:hasOBONamespace>GAZ</oboInOwl:hasOBONamespace>
        <oboInOwl:id>GAZ:00058836</oboInOwl:id>
        <rdfs:label>Kerio River Valley</rdfs:label>
    </owl:NamedIndividual>
    


    <!-- http://purl.obolibrary.org/obo/GAZ_00058840 -->

    <owl:NamedIndividual rdf:about="http://purl.obolibrary.org/obo/GAZ_00058840">
        <obo:IAO_0000115>A reservoir in south-central Ethiopia. It was created by the construction of the Koka Dam across the Awash River. It is Located in the Misraq Shewa Zone of the Oromia Region. Constructed 1960.</obo:IAO_0000115>
        <oboInOwl:hasOBONamespace>GAZ</oboInOwl:hasOBONamespace>
        <oboInOwl:id>GAZ:00058840</oboInOwl:id>
        <rdfs:label>Koka Reservoir</rdfs:label>
    </owl:NamedIndividual>
    


    <!-- http://purl.obolibrary.org/obo/GAZ_00076364 -->

    <owl:NamedIndividual rdf:about="http://purl.obolibrary.org/obo/GAZ_00076364">
        <obo:RO_0001025 rdf:resource="http://purl.obolibrary.org/obo/GAZ_00000581"/>
        <obo:IAO_0000115>A national park.</obo:IAO_0000115>
        <oboInOwl:hasOBONamespace>GAZ</oboInOwl:hasOBONamespace>
        <oboInOwl:id>GAZ:00076364</oboInOwl:id>
        <rdfs:label>Semenawi Bahri National Park</rdfs:label>
    </owl:NamedIndividual>
    


    <!-- http://purl.obolibrary.org/obo/GAZ_00076365 -->

    <owl:NamedIndividual rdf:about="http://purl.obolibrary.org/obo/GAZ_00076365">
        <obo:RO_0001025 rdf:resource="http://purl.obolibrary.org/obo/GAZ_00031068"/>
        <obo:IAO_0000115>A national park in the central coastal region of Eritrea. The Park is entirely located in the Northern Red Sea Region and includes part of the Dahlak Islands.</obo:IAO_0000115>
        <oboInOwl:hasOBONamespace>GAZ</oboInOwl:hasOBONamespace>
        <oboInOwl:id>GAZ:00076365</oboInOwl:id>
        <rdfs:label>Dahlak Marine National Park</rdfs:label>
    </owl:NamedIndividual>
    


    <!-- http://purl.obolibrary.org/obo/GAZ_00076368 -->

    <owl:NamedIndividual rdf:about="http://purl.obolibrary.org/obo/GAZ_00076368">
        <obo:RO_0001025 rdf:resource="http://purl.obolibrary.org/obo/GAZ_00052578"/>
        <obo:IAO_0000115>A national parks of Ethiopia. Located in the Semien Gondar Zone of the Amhara Region, its territory covers the Semien Mountains and includes Ras Dashan, the highest point in Ethiopia and fourth-highest in Africa. Established 1969. A World Heritage Site.</obo:IAO_0000115>
        <oboInOwl:hasOBONamespace>GAZ</oboInOwl:hasOBONamespace>
        <oboInOwl:id>GAZ:00076368</oboInOwl:id>
        <rdfs:label>Semien Mountains National Park</rdfs:label>
    </owl:NamedIndividual>
    


    <!-- http://purl.obolibrary.org/obo/GAZ_00076405 -->

    <owl:NamedIndividual rdf:about="http://purl.obolibrary.org/obo/GAZ_00076405">
        <obo:RO_0001025 rdf:resource="http://purl.obolibrary.org/obo/GAZ_00000007"/>
        <obo:IAO_0000115>A national park that lies south of Lake Naivasha in Kenya, north west of Nairobi. It includes the Fischer&apos;s Tower and Central Tower columns and Hell&apos;s Gate Gorge. The national park is also home to three geothermal power stations at Olkaria.</obo:IAO_0000115>
        <oboInOwl:hasOBONamespace>GAZ</oboInOwl:hasOBONamespace>
        <oboInOwl:id>GAZ:00076405</oboInOwl:id>
        <rdfs:label>Hell&apos;s Gate National Park</rdfs:label>
    </owl:NamedIndividual>
    


    <!-- http://purl.obolibrary.org/obo/GAZ_00076707 -->

    <owl:NamedIndividual rdf:about="http://purl.obolibrary.org/obo/GAZ_00076707">
        <obo:RO_0001025 rdf:resource="http://purl.obolibrary.org/obo/GAZ_00076708"/>
        <obo:IAO_0000115>A national park in Tanzania.</obo:IAO_0000115>
        <oboInOwl:hasOBONamespace>GAZ</oboInOwl:hasOBONamespace>
        <oboInOwl:id>GAZ:00076707</oboInOwl:id>
        <rdfs:label>Rubondo Island National Park</rdfs:label>
    </owl:NamedIndividual>
    


    <!-- http://purl.obolibrary.org/obo/GAZ_00076708 -->

    <owl:NamedIndividual rdf:about="http://purl.obolibrary.org/obo/GAZ_00076708">
        <obo:RO_0001025 rdf:resource="http://purl.obolibrary.org/obo/GAZ_00015452"/>
        <obo:IAO_0000115>An island in the SW of Lake Victoria.</obo:IAO_0000115>
        <oboInOwl:hasOBONamespace>GAZ</oboInOwl:hasOBONamespace>
        <oboInOwl:id>GAZ:00076708</oboInOwl:id>
        <rdfs:label>Rubondo Island</rdfs:label>
    </owl:NamedIndividual>
    


    <!-- http://purl.obolibrary.org/obo/GAZ_00076715 -->

    <owl:NamedIndividual rdf:about="http://purl.obolibrary.org/obo/GAZ_00076715">
        <obo:RO_0001025 rdf:resource="http://purl.obolibrary.org/obo/GAZ_00000007"/>
        <obo:IAO_0000115>A protected area in Tanzania.</obo:IAO_0000115>
        <oboInOwl:hasOBONamespace>GAZ</oboInOwl:hasOBONamespace>
        <oboInOwl:id>GAZ:00076715</oboInOwl:id>
        <rdfs:label>Uwanda Game Reserve</rdfs:label>
    </owl:NamedIndividual>
    


    <!-- http://purl.obolibrary.org/obo/GAZ_00123543 -->

    <owl:NamedIndividual rdf:about="http://purl.obolibrary.org/obo/GAZ_00123543">
        <obo:IAO_0000115>A rugged mass of mountains in Ethiopia, Eritrea (which is sometimes referred to as the Eritrean Highlands), and northern Somalia (Somaliland) in the Horn of Africa.</obo:IAO_0000115>
        <oboInOwl:hasOBONamespace>GAZ</oboInOwl:hasOBONamespace>
        <oboInOwl:id>GAZ:00123543</oboInOwl:id>
        <rdfs:label>Ethiopian Highlands</rdfs:label>
    </owl:NamedIndividual>
    


    <!-- http://purl.obolibrary.org/obo/GAZ_00123544 -->

    <owl:NamedIndividual rdf:about="http://purl.obolibrary.org/obo/GAZ_00123544">
        <obo:RO_0001025 rdf:resource="http://purl.obolibrary.org/obo/GAZ_00123543"/>
        <obo:IAO_0000115>An extension of the Ethiopian Highlands to the south. The Eritrean Highlands are drained by four major rivers towards Sudan and by several smaller rivers into the Red Sea coast of Eritrea. Flowing towards Sudan and the Nile River are the Gash and Setit Rivers while towards Sudan without reaching the Nile are the Barka and Anseba Rivers. The Eastern Escarpment of Eritrea is drained by numerous small streams.</obo:IAO_0000115>
        <oboInOwl:hasOBONamespace>GAZ</oboInOwl:hasOBONamespace>
        <oboInOwl:id>GAZ:00123544</oboInOwl:id>
        <rdfs:label>Eritrean Highlands</rdfs:label>
    </owl:NamedIndividual>
    


    <!-- http://purl.obolibrary.org/obo/GAZ_00123907 -->

    <owl:NamedIndividual rdf:about="http://purl.obolibrary.org/obo/GAZ_00123907">
        <obo:RO_0001025 rdf:resource="http://purl.obolibrary.org/obo/GAZ_00123543"/>
        <obo:IAO_0000115>An isolated, extinct silicic volcanic mountain in southeastern Ethiopia. The highest point in the Arsi Zone of the Oromia Region, and located on the border between the Hitosa and Tiyo wored. Although this mountain is located south of the Great Rift Valley, along with Mount Gugu to the north and Mount Kaka to the south, it is considered, geologically speaking, part of the Ethiopian highlands.</obo:IAO_0000115>
        <oboInOwl:hasOBONamespace>GAZ</oboInOwl:hasOBONamespace>
        <oboInOwl:id>GAZ:00123907</oboInOwl:id>
        <rdfs:label>Mount Chilalo</rdfs:label>
    </owl:NamedIndividual>
    


    <!-- http://purl.obolibrary.org/obo/GAZ_00124218 -->

    <owl:NamedIndividual rdf:about="http://purl.obolibrary.org/obo/GAZ_00124218">
        <obo:RO_0001025 rdf:resource="http://purl.obolibrary.org/obo/GAZ_00000007"/>
        <obo:IAO_0000115>A series of hills in Baringo District, Kenya.</obo:IAO_0000115>
        <oboInOwl:hasOBONamespace>GAZ</oboInOwl:hasOBONamespace>
        <oboInOwl:id>GAZ:00124218</oboInOwl:id>
        <rdfs:label>Tugen Hills</rdfs:label>
    </owl:NamedIndividual>
    


    <!-- http://purl.obolibrary.org/obo/GAZ_00124306 -->

    <owl:NamedIndividual rdf:about="http://purl.obolibrary.org/obo/GAZ_00124306">
        <obo:RO_0001025 rdf:resource="http://purl.obolibrary.org/obo/GAZ_00000007"/>
        <obo:IAO_0000115>A steep natural cliff approximately 3,000 m high, running along the western edge of the Great Rift Valley in Kenya.</obo:IAO_0000115>
        <oboInOwl:hasOBONamespace>GAZ</oboInOwl:hasOBONamespace>
        <oboInOwl:id>GAZ:00124306</oboInOwl:id>
        <rdfs:label>Mau Escarpment</rdfs:label>
    </owl:NamedIndividual>
    


    <!-- http://purl.obolibrary.org/obo/GAZ_00124307 -->

    <owl:NamedIndividual rdf:about="http://purl.obolibrary.org/obo/GAZ_00124307">
        <obo:RO_0001025 rdf:resource="http://purl.obolibrary.org/obo/GAZ_00124306"/>
        <obo:IAO_0000115>A forest complex in the Rift Valley of Kenya. It is the largest indigenous montane forest in East Africa. The Mau Forest complex has an area of 273300 ha.</obo:IAO_0000115>
        <oboInOwl:hasOBONamespace>GAZ</oboInOwl:hasOBONamespace>
        <oboInOwl:id>GAZ:00124307</oboInOwl:id>
        <rdfs:label>Mau Forest</rdfs:label>
    </owl:NamedIndividual>
    


    <!-- http://purl.obolibrary.org/obo/GAZ_00124567 -->

    <owl:NamedIndividual rdf:about="http://purl.obolibrary.org/obo/GAZ_00124567">
        <obo:RO_0001025 rdf:resource="http://purl.obolibrary.org/obo/GAZ_00015452"/>
        <oboInOwl:hasOBONamespace>GAZ</oboInOwl:hasOBONamespace>
        <oboInOwl:id>GAZ:00124567</oboInOwl:id>
        <rdfs:label>Napoleon Gulf</rdfs:label>
    </owl:NamedIndividual>
    


    <!-- http://purl.obolibrary.org/obo/GAZ_00124568 -->

    <owl:NamedIndividual rdf:about="http://purl.obolibrary.org/obo/GAZ_00124568">
        <obo:RO_0001025 rdf:resource="http://purl.obolibrary.org/obo/GAZ_00015453"/>
        <obo:IAO_0000115>The largest of the Buvuma Islands.</obo:IAO_0000115>
        <oboInOwl:hasOBONamespace>GAZ</oboInOwl:hasOBONamespace>
        <oboInOwl:id>GAZ:00124568</oboInOwl:id>
        <rdfs:label>Buvuma Island</rdfs:label>
    </owl:NamedIndividual>
    


    <!-- http://purl.obolibrary.org/obo/GAZ_00124569 -->

    <owl:NamedIndividual rdf:about="http://purl.obolibrary.org/obo/GAZ_00124569">
        <obo:RO_0001025 rdf:resource="http://purl.obolibrary.org/obo/GAZ_00015452"/>
        <obo:RO_0001025 rdf:resource="http://purl.obolibrary.org/obo/GAZ_00015453"/>
        <obo:IAO_0000115>One of the Buvuma Islands.</obo:IAO_0000115>
        <oboInOwl:hasOBONamespace>GAZ</oboInOwl:hasOBONamespace>
        <oboInOwl:id>GAZ:00124569</oboInOwl:id>
        <rdfs:label>Bugaia Island</rdfs:label>
    </owl:NamedIndividual>
    


    <!-- http://purl.obolibrary.org/obo/GAZ_00124570 -->

    <owl:NamedIndividual rdf:about="http://purl.obolibrary.org/obo/GAZ_00124570">
        <obo:RO_0001025 rdf:resource="http://purl.obolibrary.org/obo/GAZ_00015452"/>
        <obo:RO_0001025 rdf:resource="http://purl.obolibrary.org/obo/GAZ_00015453"/>
        <obo:IAO_0000115>One of the Buvuma Islands.</obo:IAO_0000115>
        <oboInOwl:hasOBONamespace>GAZ</oboInOwl:hasOBONamespace>
        <oboInOwl:id>GAZ:00124570</oboInOwl:id>
        <rdfs:label>Lingira Island</rdfs:label>
    </owl:NamedIndividual>
    


    <!-- http://purl.obolibrary.org/obo/GAZ_00124571 -->

    <owl:NamedIndividual rdf:about="http://purl.obolibrary.org/obo/GAZ_00124571">
        <obo:RO_0001025 rdf:resource="http://purl.obolibrary.org/obo/GAZ_00015452"/>
        <obo:RO_0001025 rdf:resource="http://purl.obolibrary.org/obo/GAZ_00015453"/>
        <obo:IAO_0000115>One of the Buvuma Islands.</obo:IAO_0000115>
        <oboInOwl:hasOBONamespace>GAZ</oboInOwl:hasOBONamespace>
        <oboInOwl:id>GAZ:00124571</oboInOwl:id>
        <rdfs:label>Namiti Island</rdfs:label>
    </owl:NamedIndividual>
    


    <!-- http://purl.obolibrary.org/obo/GAZ_00136138 -->

    <owl:NamedIndividual rdf:about="http://purl.obolibrary.org/obo/GAZ_00136138">
        <obo:RO_0001025 rdf:resource="http://purl.obolibrary.org/obo/GAZ_00000007"/>
        <obo:IAO_0000115>A region along the East African Rift in Tanzania, located in a spreading zone at the intersection of branches of the African and Somali tectonic plates.</obo:IAO_0000115>
        <oboInOwl:hasOBONamespace>GAZ</oboInOwl:hasOBONamespace>
        <oboInOwl:id>GAZ:00136138</oboInOwl:id>
        <rdfs:label>Crater Highlands</rdfs:label>
    </owl:NamedIndividual>
    


    <!-- http://purl.obolibrary.org/obo/GAZ_00136139 -->

    <owl:NamedIndividual rdf:about="http://purl.obolibrary.org/obo/GAZ_00136139">
        <obo:RO_0001025 rdf:resource="http://purl.obolibrary.org/obo/GAZ_00136138"/>
        <oboInOwl:hasOBONamespace>GAZ</oboInOwl:hasOBONamespace>
        <oboInOwl:id>GAZ:00136139</oboInOwl:id>
        <rdfs:label>Ela Naibori Crater</rdfs:label>
    </owl:NamedIndividual>
    


    <!-- http://purl.obolibrary.org/obo/GAZ_00136140 -->

    <owl:NamedIndividual rdf:about="http://purl.obolibrary.org/obo/GAZ_00136140">
        <obo:RO_0001025 rdf:resource="http://purl.obolibrary.org/obo/GAZ_00136138"/>
        <obo:IAO_0000115>A volcano located in Tanzania in the Crater Highlands region. It is at the southeastern edge of Lake Natron in Africa&apos;s Great Rift Valley.</obo:IAO_0000115>
        <oboInOwl:hasOBONamespace>GAZ</oboInOwl:hasOBONamespace>
        <oboInOwl:id>GAZ:00136140</oboInOwl:id>
        <rdfs:label>Gelai Volcano</rdfs:label>
    </owl:NamedIndividual>
    


    <!-- http://purl.obolibrary.org/obo/GAZ_00136141 -->

    <owl:NamedIndividual rdf:about="http://purl.obolibrary.org/obo/GAZ_00136141">
        <obo:RO_0001025 rdf:resource="http://purl.obolibrary.org/obo/GAZ_00136138"/>
        <oboInOwl:hasOBONamespace>GAZ</oboInOwl:hasOBONamespace>
        <oboInOwl:id>GAZ:00136141</oboInOwl:id>
        <rdfs:label>Meto Hills</rdfs:label>
    </owl:NamedIndividual>
    


    <!-- http://purl.obolibrary.org/obo/GAZ_00145311 -->

    <owl:NamedIndividual rdf:about="http://purl.obolibrary.org/obo/GAZ_00145311">
        <obo:IAO_0000115>A body of water on the Eritrean coastline on the Red Sea. The Gulf lies near the midpoint of the Eritrean coast, between the Foro province and the Buri Peninsula of the Ghelae&apos;lo province, both in the country&apos;s Northern Red Sea region.</obo:IAO_0000115>
        <oboInOwl:hasOBONamespace>GAZ</oboInOwl:hasOBONamespace>
        <oboInOwl:id>GAZ:00145311</oboInOwl:id>
        <rdfs:label>Gulf of Zula</rdfs:label>
    </owl:NamedIndividual>
    


    <!-- http://purl.obolibrary.org/obo/GAZ_00146201 -->

    <owl:NamedIndividual rdf:about="http://purl.obolibrary.org/obo/GAZ_00146201">
        <obo:RO_0001025 rdf:resource="http://purl.obolibrary.org/obo/GAZ_00000581"/>
        <obo:IAO_0000115>A bay on the Red Sea, off the coast of Eritrea.</obo:IAO_0000115>
        <oboInOwl:hasOBONamespace>GAZ</oboInOwl:hasOBONamespace>
        <oboInOwl:id>GAZ:00146201</oboInOwl:id>
        <rdfs:label>Amphila Bay</rdfs:label>
    </owl:NamedIndividual>
    


    <!-- http://purl.obolibrary.org/obo/GAZ_00176005 -->

    <owl:NamedIndividual rdf:about="http://purl.obolibrary.org/obo/GAZ_00176005">
        <obo:RO_0001025 rdf:resource="http://purl.obolibrary.org/obo/GAZ_00007862"/>
        <obo:IAO_0000115>An island in the northern Gulf of Aqaba off the shore of Egypt&apos;s eastern Sinai Peninsula.</obo:IAO_0000115>
        <oboInOwl:hasOBONamespace>GAZ</oboInOwl:hasOBONamespace>
        <oboInOwl:id>GAZ:00176005</oboInOwl:id>
        <rdfs:label>Pharaoh&apos;s Island</rdfs:label>
    </owl:NamedIndividual>
    


    <!-- http://purl.obolibrary.org/obo/GAZ_00193785 -->

    <owl:NamedIndividual rdf:about="http://purl.obolibrary.org/obo/GAZ_00193785">
        <obo:RO_0001025 rdf:resource="http://purl.obolibrary.org/obo/GAZ_00007520"/>
        <obo:IAO_0000115>A river. A tributary of the Jordan River.</obo:IAO_0000115>
        <oboInOwl:hasOBONamespace>GAZ</oboInOwl:hasOBONamespace>
        <oboInOwl:id>GAZ:00193785</oboInOwl:id>
        <rdfs:label>Banias River</rdfs:label>
    </owl:NamedIndividual>
    


    <!-- http://purl.obolibrary.org/obo/GAZ_00193791 -->

    <owl:NamedIndividual rdf:about="http://purl.obolibrary.org/obo/GAZ_00193791">
        <obo:IAO_0000115>The lowest nature reserve in the world, with a spectacular array of scenery near the east cost of the Dead Sea. The reserve is located within the deep Wadi Mujib gorge, which enters the Dead Sea at 410 m below sea level. The Reserve extends to the Kerak and Madaba mountains to the north and south.</obo:IAO_0000115>
        <oboInOwl:hasOBONamespace>GAZ</oboInOwl:hasOBONamespace>
        <oboInOwl:id>GAZ:00193791</oboInOwl:id>
        <rdfs:label>Mujib Nature Reserve</rdfs:label>
    </owl:NamedIndividual>
    


    <!-- http://purl.obolibrary.org/obo/GAZ_00193804 -->

    <owl:NamedIndividual rdf:about="http://purl.obolibrary.org/obo/GAZ_00193804">
        <obo:RO_0001025 rdf:resource="http://purl.obolibrary.org/obo/GAZ_00007862"/>
        <obo:IAO_0000115>A protected area located on the Red Sea south of Eilat.</obo:IAO_0000115>
        <oboInOwl:hasOBONamespace>GAZ</oboInOwl:hasOBONamespace>
        <oboInOwl:id>GAZ:00193804</oboInOwl:id>
        <rdfs:label>Coral Beach Nature Reserve</rdfs:label>
    </owl:NamedIndividual>
    


    <!-- http://purl.obolibrary.org/obo/GAZ_00193854 -->

    <owl:NamedIndividual rdf:about="http://purl.obolibrary.org/obo/GAZ_00193854">
        <obo:RO_0001025 rdf:resource="http://purl.obolibrary.org/obo/GAZ_00010533"/>
        <obo:IAO_0000115>A protected area. An archeological site. A World Heritage Site.</obo:IAO_0000115>
        <oboInOwl:hasOBONamespace>GAZ</oboInOwl:hasOBONamespace>
        <oboInOwl:id>GAZ:00193854</oboInOwl:id>
        <rdfs:label>Megiddo National Park</rdfs:label>
    </owl:NamedIndividual>
    


    <!-- http://purl.obolibrary.org/obo/GAZ_00193855 -->

    <owl:NamedIndividual rdf:about="http://purl.obolibrary.org/obo/GAZ_00193855">
        <obo:RO_0001025 rdf:resource="http://purl.obolibrary.org/obo/GAZ_00010533"/>
        <obo:IAO_0000115>A protected area. An archeological site.</obo:IAO_0000115>
        <oboInOwl:hasOBONamespace>GAZ</oboInOwl:hasOBONamespace>
        <oboInOwl:id>GAZ:00193855</oboInOwl:id>
        <rdfs:label>Ma&apos;ayan Harod National Park</rdfs:label>
    </owl:NamedIndividual>
    


    <!-- http://purl.obolibrary.org/obo/GAZ_00193856 -->

    <owl:NamedIndividual rdf:about="http://purl.obolibrary.org/obo/GAZ_00193856">
        <obo:RO_0001025 rdf:resource="http://purl.obolibrary.org/obo/GAZ_00193855"/>
        <obo:IAO_0000115>A spring. It emerges from a rocky cave on the slope of Mount Gilboa.</obo:IAO_0000115>
        <oboInOwl:hasOBONamespace>GAZ</oboInOwl:hasOBONamespace>
        <oboInOwl:id>GAZ:00193856</oboInOwl:id>
        <rdfs:label>Ma&apos;ayan Harod</rdfs:label>
    </owl:NamedIndividual>
    


    <!-- http://purl.obolibrary.org/obo/GAZ_00193866 -->

    <owl:NamedIndividual rdf:about="http://purl.obolibrary.org/obo/GAZ_00193866">
        <obo:RO_0001025 rdf:resource="http://purl.obolibrary.org/obo/GAZ_00044915"/>
        <obo:IAO_0000115>A protected area. An archeological site.</obo:IAO_0000115>
        <oboInOwl:hasOBONamespace>GAZ</oboInOwl:hasOBONamespace>
        <oboInOwl:id>GAZ:00193866</oboInOwl:id>
        <rdfs:label>Bet She&apos;an National Park</rdfs:label>
    </owl:NamedIndividual>
    


    <!-- http://purl.obolibrary.org/obo/GAZ_00193885 -->

    <owl:NamedIndividual rdf:about="http://purl.obolibrary.org/obo/GAZ_00193885">
        <obo:RO_0001025 rdf:resource="http://purl.obolibrary.org/obo/GAZ_00008742"/>
        <obo:IAO_0000115>A protected area.</obo:IAO_0000115>
        <oboInOwl:hasOBONamespace>GAZ</oboInOwl:hasOBONamespace>
        <oboInOwl:id>GAZ:00193885</oboInOwl:id>
        <rdfs:label>Hurshat Tal National Park</rdfs:label>
    </owl:NamedIndividual>
    


    <!-- http://purl.obolibrary.org/obo/GAZ_00193886 -->

    <owl:NamedIndividual rdf:about="http://purl.obolibrary.org/obo/GAZ_00193886">
        <obo:RO_0001025 rdf:resource="http://purl.obolibrary.org/obo/GAZ_00008742"/>
        <obo:IAO_0000115>A protected area.</obo:IAO_0000115>
        <oboInOwl:hasOBONamespace>GAZ</oboInOwl:hasOBONamespace>
        <oboInOwl:id>GAZ:00193886</oboInOwl:id>
        <rdfs:label>Hula Nature Reserve</rdfs:label>
    </owl:NamedIndividual>
    


    <!-- http://purl.obolibrary.org/obo/GAZ_00193951 -->

    <owl:NamedIndividual rdf:about="http://purl.obolibrary.org/obo/GAZ_00193951">
        <obo:RO_0001025 rdf:resource="http://purl.obolibrary.org/obo/GAZ_00044915"/>
        <obo:IAO_0000115>A large spit of land which now separates the North and the South basins of the Dead Sea. Entirely located in Jordan.</obo:IAO_0000115>
        <oboInOwl:hasOBONamespace>GAZ</oboInOwl:hasOBONamespace>
        <oboInOwl:id>GAZ:00193951</oboInOwl:id>
        <rdfs:label>Lisan Peninsula</rdfs:label>
    </owl:NamedIndividual>
    


    <!-- http://purl.obolibrary.org/obo/GAZ_00230329 -->

    <owl:NamedIndividual rdf:about="http://purl.obolibrary.org/obo/GAZ_00230329">
        <rdf:type rdf:resource="http://purl.obolibrary.org/obo/ENVO_00000004"/>
        <obo:RO_0001025 rdf:resource="http://purl.obolibrary.org/obo/GAZ_00000772"/>
        <obo:IAO_0000115>A district in the Anseba region of northern-central Eritrea. The capital lies at Keren City.</obo:IAO_0000115>
        <oboInOwl:hasOBONamespace>GAZ</oboInOwl:hasOBONamespace>
        <oboInOwl:id>GAZ:00230329</oboInOwl:id>
        <rdfs:label>Keren District</rdfs:label>
    </owl:NamedIndividual>
    


    <!-- http://purl.obolibrary.org/obo/GAZ_00230330 -->

    <owl:NamedIndividual rdf:about="http://purl.obolibrary.org/obo/GAZ_00230330">
        <rdf:type rdf:resource="http://purl.obolibrary.org/obo/ENVO_00000004"/>
        <obo:RO_0001025 rdf:resource="http://purl.obolibrary.org/obo/GAZ_00000772"/>
        <obo:IAO_0000115>A district in the Anseba region of northern-central Eritrea. The capital lies at Adi Tekelezan.</obo:IAO_0000115>
        <oboInOwl:hasOBONamespace>GAZ</oboInOwl:hasOBONamespace>
        <oboInOwl:id>GAZ:00230330</oboInOwl:id>
        <rdfs:label>Adi Tekelezan District</rdfs:label>
    </owl:NamedIndividual>
    


    <!-- http://purl.obolibrary.org/obo/GAZ_00230331 -->

    <owl:NamedIndividual rdf:about="http://purl.obolibrary.org/obo/GAZ_00230331">
        <rdf:type rdf:resource="http://purl.obolibrary.org/obo/ENVO_00000004"/>
        <obo:RO_0001025 rdf:resource="http://purl.obolibrary.org/obo/GAZ_00000774"/>
        <obo:IAO_0000115>A district in the Gash-Barka region of western Eritrea. The capital lies at Akurdet.</obo:IAO_0000115>
        <oboInOwl:hasOBONamespace>GAZ</oboInOwl:hasOBONamespace>
        <oboInOwl:id>GAZ:00230331</oboInOwl:id>
        <rdfs:label>Akurdet District</rdfs:label>
    </owl:NamedIndividual>
    


    <!-- http://purl.obolibrary.org/obo/GAZ_00230334 -->

    <owl:NamedIndividual rdf:about="http://purl.obolibrary.org/obo/GAZ_00230334">
        <rdf:type rdf:resource="http://purl.obolibrary.org/obo/ENVO_00000004"/>
        <obo:RO_0001025 rdf:resource="http://purl.obolibrary.org/obo/GAZ_00000774"/>
        <obo:IAO_0000115>A district in the Gash-Barka region of western Eritrea. The capital lies at Barentu.</obo:IAO_0000115>
        <oboInOwl:hasOBONamespace>GAZ</oboInOwl:hasOBONamespace>
        <oboInOwl:id>GAZ:00230334</oboInOwl:id>
        <rdfs:label>Barentu District</rdfs:label>
    </owl:NamedIndividual>
    


    <!-- http://purl.obolibrary.org/obo/GAZ_00230337 -->

    <owl:NamedIndividual rdf:about="http://purl.obolibrary.org/obo/GAZ_00230337">
        <oboInOwl:hasOBONamespace>GAZ</oboInOwl:hasOBONamespace>
        <oboInOwl:id>GAZ:00230337</oboInOwl:id>
        <rdfs:label>Sarana River</rdfs:label>
    </owl:NamedIndividual>
    


    <!-- http://purl.obolibrary.org/obo/GAZ_00230338 -->

    <owl:NamedIndividual rdf:about="http://purl.obolibrary.org/obo/GAZ_00230338">
        <oboInOwl:hasOBONamespace>GAZ</oboInOwl:hasOBONamespace>
        <oboInOwl:id>GAZ:00230338</oboInOwl:id>
        <rdfs:label>Balasa River</rdfs:label>
    </owl:NamedIndividual>
    


    <!-- http://purl.obolibrary.org/obo/GAZ_00230339 -->

    <owl:NamedIndividual rdf:about="http://purl.obolibrary.org/obo/GAZ_00230339">
        <obo:IAO_0000115>A river. A tributary of the Mareb River in Ethiopia.</obo:IAO_0000115>
        <oboInOwl:hasOBONamespace>GAZ</oboInOwl:hasOBONamespace>
        <oboInOwl:id>GAZ:00230339</oboInOwl:id>
        <rdfs:label>Mai Shawesh River</rdfs:label>
    </owl:NamedIndividual>
    


    <!-- http://purl.obolibrary.org/obo/GAZ_00230340 -->

    <owl:NamedIndividual rdf:about="http://purl.obolibrary.org/obo/GAZ_00230340">
        <obo:IAO_0000115>A river. A tributary of the Mareb River in Ethiopia.</obo:IAO_0000115>
        <oboInOwl:hasOBONamespace>GAZ</oboInOwl:hasOBONamespace>
        <oboInOwl:id>GAZ:00230340</oboInOwl:id>
        <rdfs:label>&apos;Engweya River</rdfs:label>
    </owl:NamedIndividual>
    


    <!-- http://purl.obolibrary.org/obo/GAZ_00230341 -->

    <owl:NamedIndividual rdf:about="http://purl.obolibrary.org/obo/GAZ_00230341">
        <obo:RO_0001025 rdf:resource="http://purl.obolibrary.org/obo/GAZ_00051205"/>
        <obo:RO_0001025 rdf:resource="http://purl.obolibrary.org/obo/GAZ_10000775"/>
        <obo:IAO_0000115>A lake. Located in the Northern Red Sea Region, Lake Kulul lies in the Eritrean portion of the Afar Depression.</obo:IAO_0000115>
        <oboInOwl:hasOBONamespace>GAZ</oboInOwl:hasOBONamespace>
        <oboInOwl:id>GAZ:00230341</oboInOwl:id>
        <rdfs:label>Lake Kulul</rdfs:label>
    </owl:NamedIndividual>
    


    <!-- http://purl.obolibrary.org/obo/GAZ_00230345 -->

    <owl:NamedIndividual rdf:about="http://purl.obolibrary.org/obo/GAZ_00230345">
        <obo:RO_0001025 rdf:resource="http://purl.obolibrary.org/obo/GAZ_00000773"/>
        <obo:IAO_0000115>The capital city and largest settlement in Eritrea.</obo:IAO_0000115>
        <oboInOwl:hasOBONamespace>GAZ</oboInOwl:hasOBONamespace>
        <oboInOwl:id>GAZ:00230345</oboInOwl:id>
        <rdfs:label>Asmara</rdfs:label>
    </owl:NamedIndividual>
    


    <!-- http://purl.obolibrary.org/obo/GAZ_00230346 -->

    <owl:NamedIndividual rdf:about="http://purl.obolibrary.org/obo/GAZ_00230346">
        <obo:RO_0001025 rdf:resource="http://purl.obolibrary.org/obo/GAZ_00031064"/>
        <obo:IAO_0000115>A peninsula that extends from central Eritrea north into the Red Sea. To its west lies the Gulf of Zula.</obo:IAO_0000115>
        <oboInOwl:hasOBONamespace>GAZ</oboInOwl:hasOBONamespace>
        <oboInOwl:id>GAZ:00230346</oboInOwl:id>
        <rdfs:label>Buri Peninsula</rdfs:label>
    </owl:NamedIndividual>
    


    <!-- http://purl.obolibrary.org/obo/GAZ_00230347 -->

    <owl:NamedIndividual rdf:about="http://purl.obolibrary.org/obo/GAZ_00230347">
        <obo:RO_0001025 rdf:resource="http://purl.obolibrary.org/obo/GAZ_10000775"/>
        <obo:IAO_0000115>A seasonal river in Eritrea. This river passes outside the town of Ghinda.</obo:IAO_0000115>
        <oboInOwl:hasOBONamespace>GAZ</oboInOwl:hasOBONamespace>
        <oboInOwl:id>GAZ:00230347</oboInOwl:id>
        <rdfs:label>Damas River</rdfs:label>
    </owl:NamedIndividual>
    


    <!-- http://purl.obolibrary.org/obo/GAZ_00230349 -->

    <owl:NamedIndividual rdf:about="http://purl.obolibrary.org/obo/GAZ_00230349">
        <obo:RO_0001025 rdf:resource="http://purl.obolibrary.org/obo/GAZ_10000775"/>
        <obo:IAO_0000115>A seasonal river in Eritrea. The river ends north of Massawa into the Red Sea. Prior to its end the river merges with the Wokiro River.</obo:IAO_0000115>
        <oboInOwl:hasOBONamespace>GAZ</oboInOwl:hasOBONamespace>
        <oboInOwl:id>GAZ:00230349</oboInOwl:id>
        <rdfs:label>Wadi Laba River</rdfs:label>
    </owl:NamedIndividual>
    


    <!-- http://purl.obolibrary.org/obo/GAZ_00230365 -->

    <owl:NamedIndividual rdf:about="http://purl.obolibrary.org/obo/GAZ_00230365">
        <obo:IAO_0000115>A river of southern Ethiopia. Located inside Omo National Park, it is a tributary of the Omo River.</obo:IAO_0000115>
        <oboInOwl:hasOBONamespace>GAZ</oboInOwl:hasOBONamespace>
        <oboInOwl:id>GAZ:00230365</oboInOwl:id>
        <rdfs:label>Mui River</rdfs:label>
    </owl:NamedIndividual>
    


    <!-- http://purl.obolibrary.org/obo/GAZ_00230369 -->

    <owl:NamedIndividual rdf:about="http://purl.obolibrary.org/obo/GAZ_00230369">
        <obo:IAO_0000115>A river of southern Ethiopia, entirely located in the Debub Omo Zone of the Southern Nations, Nationalities, and People&apos;s Region. It is a tributary of the Omo River.</obo:IAO_0000115>
        <oboInOwl:hasOBONamespace>GAZ</oboInOwl:hasOBONamespace>
        <oboInOwl:id>GAZ:00230369</oboInOwl:id>
        <rdfs:label>Mago River</rdfs:label>
    </owl:NamedIndividual>
    


    <!-- http://purl.obolibrary.org/obo/GAZ_00230372 -->

    <owl:NamedIndividual rdf:about="http://purl.obolibrary.org/obo/GAZ_00230372">
        <obo:IAO_0000115>A hydroelectric dam. Completed 2004.</obo:IAO_0000115>
        <oboInOwl:hasOBONamespace>GAZ</oboInOwl:hasOBONamespace>
        <oboInOwl:id>GAZ:00230372</oboInOwl:id>
        <rdfs:label>Gojeb Dam</rdfs:label>
    </owl:NamedIndividual>
    


    <!-- http://purl.obolibrary.org/obo/GAZ_00230373 -->

    <owl:NamedIndividual rdf:about="http://purl.obolibrary.org/obo/GAZ_00230373">
        <obo:RO_0001025 rdf:resource="http://purl.obolibrary.org/obo/GAZ_00052567"/>
        <obo:IAO_0000115>A river. A tributary of the Omo River.</obo:IAO_0000115>
        <oboInOwl:hasOBONamespace>GAZ</oboInOwl:hasOBONamespace>
        <oboInOwl:id>GAZ:00230373</oboInOwl:id>
        <rdfs:label>Wabi River</rdfs:label>
    </owl:NamedIndividual>
    


    <!-- http://purl.obolibrary.org/obo/GAZ_00230374 -->

    <owl:NamedIndividual rdf:about="http://purl.obolibrary.org/obo/GAZ_00230374">
        <obo:RO_0001025 rdf:resource="http://purl.obolibrary.org/obo/GAZ_00052567"/>
        <obo:IAO_0000115>A hydroelectric dam.</obo:IAO_0000115>
        <oboInOwl:hasOBONamespace>GAZ</oboInOwl:hasOBONamespace>
        <oboInOwl:id>GAZ:00230374</oboInOwl:id>
        <rdfs:label>Gibe III Dam</rdfs:label>
    </owl:NamedIndividual>
    


    <!-- http://purl.obolibrary.org/obo/GAZ_00230375 -->

    <owl:NamedIndividual rdf:about="http://purl.obolibrary.org/obo/GAZ_00230375">
        <obo:IAO_0000115>A hydroelectric dam. Constructed 1986-2004.</obo:IAO_0000115>
        <oboInOwl:hasOBONamespace>GAZ</oboInOwl:hasOBONamespace>
        <oboInOwl:id>GAZ:00230375</oboInOwl:id>
        <rdfs:label>Gilgel Gibe Dam</rdfs:label>
    </owl:NamedIndividual>
    


    <!-- http://purl.obolibrary.org/obo/GAZ_00230376 -->

    <owl:NamedIndividual rdf:about="http://purl.obolibrary.org/obo/GAZ_00230376">
        <obo:RO_0001025 rdf:resource="http://purl.obolibrary.org/obo/GAZ_00052531"/>
        <obo:IAO_0000115>A forest located in Ethiopia within a portion of the Bale Mountains.</obo:IAO_0000115>
        <oboInOwl:hasOBONamespace>GAZ</oboInOwl:hasOBONamespace>
        <oboInOwl:id>GAZ:00230376</oboInOwl:id>
        <rdfs:label>Harenna Forest</rdfs:label>
    </owl:NamedIndividual>
    


    <!-- http://purl.obolibrary.org/obo/GAZ_00230429 -->

    <owl:NamedIndividual rdf:about="http://purl.obolibrary.org/obo/GAZ_00230429">
        <obo:IAO_0000115>A river of south-central Ethiopia. It rises on the southwestern slopes of Mount Gurage, flowing south along the western side of the Great Rift Valley, to empty into Lake Abaya.</obo:IAO_0000115>
        <oboInOwl:hasOBONamespace>GAZ</oboInOwl:hasOBONamespace>
        <oboInOwl:id>GAZ:00230429</oboInOwl:id>
        <rdfs:label>Bilate River</rdfs:label>
    </owl:NamedIndividual>
    


    <!-- http://purl.obolibrary.org/obo/GAZ_00230463 -->

    <owl:NamedIndividual rdf:about="http://purl.obolibrary.org/obo/GAZ_00230463">
        <obo:IAO_0000115>A river in central Ethiopia. It empties into Lake Zway.</obo:IAO_0000115>
        <oboInOwl:hasOBONamespace>GAZ</oboInOwl:hasOBONamespace>
        <oboInOwl:id>GAZ:00230463</oboInOwl:id>
        <rdfs:label>Meki River</rdfs:label>
    </owl:NamedIndividual>
    


    <!-- http://purl.obolibrary.org/obo/GAZ_00234085 -->

    <owl:NamedIndividual rdf:about="http://purl.obolibrary.org/obo/GAZ_00234085">
        <obo:IAO_0000115>A hydroelectric dam. Located at the Ruzizi River outlet from Lake Kivu. Constructed 1958.</obo:IAO_0000115>
        <oboInOwl:hasOBONamespace>GAZ</oboInOwl:hasOBONamespace>
        <oboInOwl:id>GAZ:00234085</oboInOwl:id>
        <rdfs:label>Ruzizi I Hydroelectric Dam</rdfs:label>
    </owl:NamedIndividual>
    


    <!-- http://purl.obolibrary.org/obo/GAZ_00234089 -->

    <owl:NamedIndividual rdf:about="http://purl.obolibrary.org/obo/GAZ_00234089">
        <obo:IAO_0000115>Water falls.</obo:IAO_0000115>
        <oboInOwl:hasOBONamespace>GAZ</oboInOwl:hasOBONamespace>
        <oboInOwl:id>GAZ:00234089</oboInOwl:id>
        <rdfs:label>Chutes de la Kagera</rdfs:label>
    </owl:NamedIndividual>
    


    <!-- http://purl.obolibrary.org/obo/GAZ_00235791 -->

    <owl:NamedIndividual rdf:about="http://purl.obolibrary.org/obo/GAZ_00235791">
        <obo:IAO_0000115>A river. A tributary of the Kagera River.</obo:IAO_0000115>
        <oboInOwl:hasOBONamespace>GAZ</oboInOwl:hasOBONamespace>
        <oboInOwl:id>GAZ:00235791</oboInOwl:id>
        <rdfs:label>Muvumba River</rdfs:label>
    </owl:NamedIndividual>
    


    <!-- http://purl.obolibrary.org/obo/GAZ_00235792 -->

    <owl:NamedIndividual rdf:about="http://purl.obolibrary.org/obo/GAZ_00235792">
        <oboInOwl:hasOBONamespace>GAZ</oboInOwl:hasOBONamespace>
        <oboInOwl:id>GAZ:00235792</oboInOwl:id>
        <rdfs:label>Karangaza River</rdfs:label>
    </owl:NamedIndividual>
    


    <!-- http://purl.obolibrary.org/obo/GAZ_00235793 -->

    <owl:NamedIndividual rdf:about="http://purl.obolibrary.org/obo/GAZ_00235793">
        <oboInOwl:hasOBONamespace>GAZ</oboInOwl:hasOBONamespace>
        <oboInOwl:id>GAZ:00235793</oboInOwl:id>
        <rdfs:label>Kamiramugezi River</rdfs:label>
    </owl:NamedIndividual>
    


    <!-- http://purl.obolibrary.org/obo/GAZ_00235795 -->

    <owl:NamedIndividual rdf:about="http://purl.obolibrary.org/obo/GAZ_00235795">
        <obo:IAO_0000115>A river flowing into Lake Kivu.</obo:IAO_0000115>
        <oboInOwl:hasOBONamespace>GAZ</oboInOwl:hasOBONamespace>
        <oboInOwl:id>GAZ:00235795</oboInOwl:id>
        <rdfs:label>Kalundura River</rdfs:label>
    </owl:NamedIndividual>
    


    <!-- http://purl.obolibrary.org/obo/GAZ_00236097 -->

    <owl:NamedIndividual rdf:about="http://purl.obolibrary.org/obo/GAZ_00236097">
        <obo:RO_0001025 rdf:resource="http://purl.obolibrary.org/obo/GAZ_00000007"/>
        <obo:IAO_0000115>An arid part of the Great Rift Valley in Kenya, directly south of Lake Turkana. The valley is floored by a seasonal stream complex, the Suguta River, that terminates in the seasonal playa Lake Alablab. Lake Logipi, a saline, alkaline lake lies at the northern end of the valley, where it is separated from Lake Turkana by a complex series of volcanoes called the Barrier.</obo:IAO_0000115>
        <oboInOwl:hasOBONamespace>GAZ</oboInOwl:hasOBONamespace>
        <oboInOwl:id>GAZ:00236097</oboInOwl:id>
        <rdfs:label>Suguta Valley</rdfs:label>
    </owl:NamedIndividual>
    


    <!-- http://purl.obolibrary.org/obo/GAZ_00236098 -->

    <owl:NamedIndividual rdf:about="http://purl.obolibrary.org/obo/GAZ_00236098">
        <obo:RO_0001025 rdf:resource="http://purl.obolibrary.org/obo/GAZ_00236097"/>
        <obo:IAO_0000115>A seasonal playa lake.</obo:IAO_0000115>
        <oboInOwl:hasOBONamespace>GAZ</oboInOwl:hasOBONamespace>
        <oboInOwl:id>GAZ:00236098</oboInOwl:id>
        <rdfs:label>Lake Alablab</rdfs:label>
    </owl:NamedIndividual>
    


    <!-- http://purl.obolibrary.org/obo/GAZ_00236099 -->

    <owl:NamedIndividual rdf:about="http://purl.obolibrary.org/obo/GAZ_00236099">
        <obo:RO_0001025 rdf:resource="http://purl.obolibrary.org/obo/GAZ_00236097"/>
        <obo:IAO_0000115>An intermittent river.</obo:IAO_0000115>
        <oboInOwl:hasOBONamespace>GAZ</oboInOwl:hasOBONamespace>
        <oboInOwl:id>GAZ:00236099</oboInOwl:id>
        <rdfs:label>Suguta River</rdfs:label>
    </owl:NamedIndividual>
    


    <!-- http://purl.obolibrary.org/obo/GAZ_00236105 -->

    <owl:NamedIndividual rdf:about="http://purl.obolibrary.org/obo/GAZ_00236105">
        <obo:RO_0001025 rdf:resource="http://purl.obolibrary.org/obo/GAZ_00000007"/>
        <obo:IAO_0000115>A fault-scarp caused by to post-Miocene faulting and there are Miocene beds visible. The escarpment is part of the western wall of the Great Rift Valley.</obo:IAO_0000115>
        <oboInOwl:hasOBONamespace>GAZ</oboInOwl:hasOBONamespace>
        <oboInOwl:id>GAZ:00236105</oboInOwl:id>
        <rdfs:label>Elgeyo Escarpment</rdfs:label>
    </owl:NamedIndividual>
    


    <!-- http://purl.obolibrary.org/obo/GAZ_00236116 -->

    <owl:NamedIndividual rdf:about="http://purl.obolibrary.org/obo/GAZ_00236116">
        <obo:RO_0001025 rdf:resource="http://purl.obolibrary.org/obo/GAZ_00000007"/>
        <obo:IAO_0000115>Peaks in a ridge along the Great Rift Valley, located southwest near Nairobi, in southern Kenya.</obo:IAO_0000115>
        <oboInOwl:hasOBONamespace>GAZ</oboInOwl:hasOBONamespace>
        <oboInOwl:id>GAZ:00236116</oboInOwl:id>
        <rdfs:label>Ngong Hills</rdfs:label>
    </owl:NamedIndividual>
    


    <!-- http://purl.obolibrary.org/obo/GAZ_00236121 -->

    <owl:NamedIndividual rdf:about="http://purl.obolibrary.org/obo/GAZ_00236121">
        <rdf:type rdf:resource="http://purl.obolibrary.org/obo/ENVO_00000100"/>
        <rdf:type rdf:resource="http://purl.obolibrary.org/obo/ENVO_00000479"/>
        <obo:RO_0001025 rdf:resource="http://purl.obolibrary.org/obo/GAZ_00076405"/>
        <obo:IAO_0000115>A gorge. A former outlet of Lake Naivasha.</obo:IAO_0000115>
        <oboInOwl:hasOBONamespace>GAZ</oboInOwl:hasOBONamespace>
        <oboInOwl:id>GAZ:00236121</oboInOwl:id>
        <rdfs:label>Njorowa Gorge</rdfs:label>
    </owl:NamedIndividual>
    


    <!-- http://purl.obolibrary.org/obo/GAZ_00236122 -->

    <owl:NamedIndividual rdf:about="http://purl.obolibrary.org/obo/GAZ_00236122">
        <obo:RO_0001025 rdf:resource="http://purl.obolibrary.org/obo/GAZ_00000007"/>
        <obo:IAO_0000115>A highland area of lush green rolling hills at the edge of the Great Rift Valley in the Rift Valley Province of Kenya.</obo:IAO_0000115>
        <oboInOwl:hasOBONamespace>GAZ</oboInOwl:hasOBONamespace>
        <oboInOwl:id>GAZ:00236122</oboInOwl:id>
        <rdfs:label>Nandi Hills</rdfs:label>
    </owl:NamedIndividual>
    


    <!-- http://purl.obolibrary.org/obo/GAZ_00236170 -->

    <owl:NamedIndividual rdf:about="http://purl.obolibrary.org/obo/GAZ_00236170">
        <obo:RO_0001025 rdf:resource="http://purl.obolibrary.org/obo/GAZ_00052895"/>
        <obo:IAO_0000115>A bay.</obo:IAO_0000115>
        <oboInOwl:hasOBONamespace>GAZ</oboInOwl:hasOBONamespace>
        <oboInOwl:id>GAZ:00236170</oboInOwl:id>
        <rdfs:label>Naya Bay</rdfs:label>
    </owl:NamedIndividual>
    


    <!-- http://purl.obolibrary.org/obo/GAZ_00236171 -->

    <owl:NamedIndividual rdf:about="http://purl.obolibrary.org/obo/GAZ_00236171">
        <obo:RO_0001025 rdf:resource="http://purl.obolibrary.org/obo/GAZ_00052895"/>
        <obo:IAO_0000115>A bay.</obo:IAO_0000115>
        <oboInOwl:hasOBONamespace>GAZ</oboInOwl:hasOBONamespace>
        <oboInOwl:id>GAZ:00236171</oboInOwl:id>
        <rdfs:label>Nyakach Bay</rdfs:label>
    </owl:NamedIndividual>
    


    <!-- http://purl.obolibrary.org/obo/GAZ_00236172 -->

    <owl:NamedIndividual rdf:about="http://purl.obolibrary.org/obo/GAZ_00236172">
        <obo:RO_0001025 rdf:resource="http://purl.obolibrary.org/obo/GAZ_00052895"/>
        <obo:IAO_0000115>A bay.</obo:IAO_0000115>
        <oboInOwl:hasOBONamespace>GAZ</oboInOwl:hasOBONamespace>
        <oboInOwl:id>GAZ:00236172</oboInOwl:id>
        <rdfs:label>Osodo Bay</rdfs:label>
    </owl:NamedIndividual>
    


    <!-- http://purl.obolibrary.org/obo/GAZ_00236173 -->

    <owl:NamedIndividual rdf:about="http://purl.obolibrary.org/obo/GAZ_00236173">
        <obo:RO_0001025 rdf:resource="http://purl.obolibrary.org/obo/GAZ_00052895"/>
        <obo:IAO_0000115>A bay.</obo:IAO_0000115>
        <oboInOwl:hasOBONamespace>GAZ</oboInOwl:hasOBONamespace>
        <oboInOwl:id>GAZ:00236173</oboInOwl:id>
        <rdfs:label>Kendu Bay</rdfs:label>
    </owl:NamedIndividual>
    


    <!-- http://purl.obolibrary.org/obo/GAZ_00236174 -->

    <owl:NamedIndividual rdf:about="http://purl.obolibrary.org/obo/GAZ_00236174">
        <obo:RO_0001025 rdf:resource="http://purl.obolibrary.org/obo/GAZ_00052895"/>
        <obo:IAO_0000115>A bay.</obo:IAO_0000115>
        <oboInOwl:hasOBONamespace>GAZ</oboInOwl:hasOBONamespace>
        <oboInOwl:id>GAZ:00236174</oboInOwl:id>
        <rdfs:label>Ruri Bay</rdfs:label>
    </owl:NamedIndividual>
    


    <!-- http://purl.obolibrary.org/obo/GAZ_00236175 -->

    <owl:NamedIndividual rdf:about="http://purl.obolibrary.org/obo/GAZ_00236175">
        <obo:RO_0001025 rdf:resource="http://purl.obolibrary.org/obo/GAZ_00052895"/>
        <obo:IAO_0000115>A bay.</obo:IAO_0000115>
        <oboInOwl:hasOBONamespace>GAZ</oboInOwl:hasOBONamespace>
        <oboInOwl:id>GAZ:00236175</oboInOwl:id>
        <rdfs:label>Mirunda Bay</rdfs:label>
    </owl:NamedIndividual>
    


    <!-- http://purl.obolibrary.org/obo/GAZ_00236176 -->

    <owl:NamedIndividual rdf:about="http://purl.obolibrary.org/obo/GAZ_00236176">
        <obo:RO_0001025 rdf:resource="http://purl.obolibrary.org/obo/GAZ_00052895"/>
        <obo:IAO_0000115>A bay.</obo:IAO_0000115>
        <oboInOwl:hasOBONamespace>GAZ</oboInOwl:hasOBONamespace>
        <oboInOwl:id>GAZ:00236176</oboInOwl:id>
        <rdfs:label>Olambwe Bay</rdfs:label>
    </owl:NamedIndividual>
    


    <!-- http://purl.obolibrary.org/obo/GAZ_00236183 -->

    <owl:NamedIndividual rdf:about="http://purl.obolibrary.org/obo/GAZ_00236183">
        <obo:RO_0001025 rdf:resource="http://purl.obolibrary.org/obo/GAZ_00008411"/>
        <obo:IAO_0000115>An alkaline hot spring running into Lake Bogoria.</obo:IAO_0000115>
        <oboInOwl:hasOBONamespace>GAZ</oboInOwl:hasOBONamespace>
        <oboInOwl:id>GAZ:00236183</oboInOwl:id>
        <rdfs:label>Loburu</rdfs:label>
    </owl:NamedIndividual>
    


    <!-- http://purl.obolibrary.org/obo/GAZ_00236184 -->

    <owl:NamedIndividual rdf:about="http://purl.obolibrary.org/obo/GAZ_00236184">
        <obo:RO_0001025 rdf:resource="http://purl.obolibrary.org/obo/GAZ_00008411"/>
        <obo:IAO_0000115>An alkaline hot spring running into Lake Bogoria.</obo:IAO_0000115>
        <oboInOwl:hasOBONamespace>GAZ</oboInOwl:hasOBONamespace>
        <oboInOwl:id>GAZ:00236184</oboInOwl:id>
        <rdfs:label>Chemurkeu</rdfs:label>
    </owl:NamedIndividual>
    


    <!-- http://purl.obolibrary.org/obo/GAZ_00236185 -->

    <owl:NamedIndividual rdf:about="http://purl.obolibrary.org/obo/GAZ_00236185">
        <obo:RO_0001025 rdf:resource="http://purl.obolibrary.org/obo/GAZ_00008411"/>
        <obo:IAO_0000115>A group of alkaline hot spring running into Lake Bogoria.</obo:IAO_0000115>
        <oboInOwl:hasOBONamespace>GAZ</oboInOwl:hasOBONamespace>
        <oboInOwl:id>GAZ:00236185</oboInOwl:id>
        <rdfs:label>Southern group of hot springs</rdfs:label>
    </owl:NamedIndividual>
    


    <!-- http://purl.obolibrary.org/obo/GAZ_00236186 -->

    <owl:NamedIndividual rdf:about="http://purl.obolibrary.org/obo/GAZ_00236186">
        <obo:RO_0001025 rdf:resource="http://purl.obolibrary.org/obo/GAZ_00236185"/>
        <obo:IAO_0000115>An alkaline hot spring running into Lake Bogoria.</obo:IAO_0000115>
        <oboInOwl:hasOBONamespace>GAZ</oboInOwl:hasOBONamespace>
        <oboInOwl:id>GAZ:00236186</oboInOwl:id>
        <rdfs:label>Ng&apos;wasis</rdfs:label>
    </owl:NamedIndividual>
    


    <!-- http://purl.obolibrary.org/obo/GAZ_00236187 -->

    <owl:NamedIndividual rdf:about="http://purl.obolibrary.org/obo/GAZ_00236187">
        <obo:RO_0001025 rdf:resource="http://purl.obolibrary.org/obo/GAZ_00236185"/>
        <obo:IAO_0000115>An alkaline hot spring running into Lake Bogoria.</obo:IAO_0000115>
        <oboInOwl:hasOBONamespace>GAZ</oboInOwl:hasOBONamespace>
        <oboInOwl:id>GAZ:00236187</oboInOwl:id>
        <rdfs:label>Koibobei</rdfs:label>
    </owl:NamedIndividual>
    


    <!-- http://purl.obolibrary.org/obo/GAZ_00236188 -->

    <owl:NamedIndividual rdf:about="http://purl.obolibrary.org/obo/GAZ_00236188">
        <obo:RO_0001025 rdf:resource="http://purl.obolibrary.org/obo/GAZ_00236185"/>
        <obo:IAO_0000115>An alkaline hot spring running into Lake Bogoria.</obo:IAO_0000115>
        <oboInOwl:hasOBONamespace>GAZ</oboInOwl:hasOBONamespace>
        <oboInOwl:id>GAZ:00236188</oboInOwl:id>
        <rdfs:label>Losaramat</rdfs:label>
    </owl:NamedIndividual>
    


    <!-- http://purl.obolibrary.org/obo/GAZ_00236192 -->

    <owl:NamedIndividual rdf:about="http://purl.obolibrary.org/obo/GAZ_00236192">
        <obo:RO_0001025 rdf:resource="http://purl.obolibrary.org/obo/GAZ_00000007"/>
        <obo:IAO_0000115>An escarpment in southern Kenya. The escarpment is around 50 km long and elongated in N-W direction. Its northern edge approximately 120 km southwest of Nairobi, while the southern edge is near the Tanzanian border, at the northwestern corner of Lake Natron. The southern Ewaso Ngiro river flows along the foot of the escarpment, while Loita Hills are located west of the escarpment . The escarpment forms the western wall of the Great Rift Valley.</obo:IAO_0000115>
        <oboInOwl:hasOBONamespace>GAZ</oboInOwl:hasOBONamespace>
        <oboInOwl:id>GAZ:00236192</oboInOwl:id>
        <rdfs:label>Nguruman Escarpment</rdfs:label>
    </owl:NamedIndividual>
    


    <!-- http://purl.obolibrary.org/obo/GAZ_00236193 -->

    <owl:NamedIndividual rdf:about="http://purl.obolibrary.org/obo/GAZ_00236193">
        <obo:RO_0001025 rdf:resource="http://purl.obolibrary.org/obo/GAZ_00236192"/>
        <obo:IAO_0000115>A protected area.</obo:IAO_0000115>
        <oboInOwl:hasOBONamespace>GAZ</oboInOwl:hasOBONamespace>
        <oboInOwl:id>GAZ:00236193</oboInOwl:id>
        <rdfs:label>Shompole Conservancy</rdfs:label>
    </owl:NamedIndividual>
    


    <!-- http://purl.obolibrary.org/obo/GAZ_00236194 -->

    <owl:NamedIndividual rdf:about="http://purl.obolibrary.org/obo/GAZ_00236194">
        <obo:IAO_0000115>A river in Rift Valley Province, Kenya. It flows northward into Lake Turkana.</obo:IAO_0000115>
        <oboInOwl:hasOBONamespace>GAZ</oboInOwl:hasOBONamespace>
        <oboInOwl:id>GAZ:00236194</oboInOwl:id>
        <rdfs:label>Kerio River</rdfs:label>
    </owl:NamedIndividual>
    


    <!-- http://purl.obolibrary.org/obo/GAZ_00236202 -->

    <owl:NamedIndividual rdf:about="http://purl.obolibrary.org/obo/GAZ_00236202">
        <obo:IAO_0000115>A hydroelectric plant.</obo:IAO_0000115>
        <oboInOwl:hasOBONamespace>GAZ</oboInOwl:hasOBONamespace>
        <oboInOwl:id>GAZ:00236202</oboInOwl:id>
        <rdfs:label>Turkwel Hydro Power Plant</rdfs:label>
    </owl:NamedIndividual>
    


    <!-- http://purl.obolibrary.org/obo/GAZ_00236239 -->

    <owl:NamedIndividual rdf:about="http://purl.obolibrary.org/obo/GAZ_00236239">
        <obo:RO_0001025 rdf:resource="http://purl.obolibrary.org/obo/GAZ_00136138"/>
        <obo:IAO_0000115>A lake.</obo:IAO_0000115>
        <oboInOwl:hasOBONamespace>GAZ</oboInOwl:hasOBONamespace>
        <oboInOwl:id>GAZ:00236239</oboInOwl:id>
        <rdfs:label>Lake Kitangiri</rdfs:label>
    </owl:NamedIndividual>
    


    <!-- http://purl.obolibrary.org/obo/GAZ_00236354 -->

    <owl:NamedIndividual rdf:about="http://purl.obolibrary.org/obo/GAZ_00236354">
        <obo:RO_0001025 rdf:resource="http://purl.obolibrary.org/obo/GAZ_00015452"/>
        <obo:IAO_0000115>An island in Lake Victoria claimed by both Uganda and Kenya.</obo:IAO_0000115>
        <oboInOwl:hasOBONamespace>GAZ</oboInOwl:hasOBONamespace>
        <oboInOwl:id>GAZ:00236354</oboInOwl:id>
        <rdfs:label>Migingo Island</rdfs:label>
    </owl:NamedIndividual>
    


    <!-- http://purl.obolibrary.org/obo/GAZ_00236355 -->

    <owl:NamedIndividual rdf:about="http://purl.obolibrary.org/obo/GAZ_00236355">
        <obo:RO_0001025 rdf:resource="http://purl.obolibrary.org/obo/GAZ_00015452"/>
        <obo:IAO_0000115>A Kenyan island whose westerly most point was used to demarcate the border between Kenya and Uganda just after parallel 1 degree in Lake Victoria.</obo:IAO_0000115>
        <oboInOwl:hasOBONamespace>GAZ</oboInOwl:hasOBONamespace>
        <oboInOwl:id>GAZ:00236355</oboInOwl:id>
        <rdfs:label>Pyramid Island</rdfs:label>
    </owl:NamedIndividual>
    


    <!-- http://purl.obolibrary.org/obo/GAZ_00236356 -->

    <owl:NamedIndividual rdf:about="http://purl.obolibrary.org/obo/GAZ_00236356">
        <obo:RO_0001025 rdf:resource="http://purl.obolibrary.org/obo/GAZ_00015452"/>
        <obo:IAO_0000115>An island.</obo:IAO_0000115>
        <oboInOwl:hasOBONamespace>GAZ</oboInOwl:hasOBONamespace>
        <oboInOwl:id>GAZ:00236356</oboInOwl:id>
        <rdfs:label>Ilemba island</rdfs:label>
    </owl:NamedIndividual>
    


    <!-- http://purl.obolibrary.org/obo/GAZ_00236357 -->

    <owl:NamedIndividual rdf:about="http://purl.obolibrary.org/obo/GAZ_00236357">
        <obo:RO_0001025 rdf:resource="http://purl.obolibrary.org/obo/GAZ_00015452"/>
        <obo:IAO_0000115>An island.</obo:IAO_0000115>
        <oboInOwl:hasOBONamespace>GAZ</oboInOwl:hasOBONamespace>
        <oboInOwl:id>GAZ:00236357</oboInOwl:id>
        <rdfs:label>Sumba Island</rdfs:label>
    </owl:NamedIndividual>
    


    <!-- http://purl.obolibrary.org/obo/GAZ_00236358 -->

    <owl:NamedIndividual rdf:about="http://purl.obolibrary.org/obo/GAZ_00236358">
        <obo:RO_0001025 rdf:resource="http://purl.obolibrary.org/obo/GAZ_00015452"/>
        <obo:IAO_0000115>An island in Lake Victoria.</obo:IAO_0000115>
        <oboInOwl:hasOBONamespace>GAZ</oboInOwl:hasOBONamespace>
        <oboInOwl:id>GAZ:00236358</oboInOwl:id>
        <rdfs:label>Mageta Island</rdfs:label>
    </owl:NamedIndividual>
    


    <!-- http://purl.obolibrary.org/obo/GAZ_00236359 -->

    <owl:NamedIndividual rdf:about="http://purl.obolibrary.org/obo/GAZ_00236359">
        <obo:RO_0001025 rdf:resource="http://purl.obolibrary.org/obo/GAZ_00015452"/>
        <obo:IAO_0000115>An island.</obo:IAO_0000115>
        <oboInOwl:hasOBONamespace>GAZ</oboInOwl:hasOBONamespace>
        <oboInOwl:id>GAZ:00236359</oboInOwl:id>
        <rdfs:label>Kiringiti Island</rdfs:label>
    </owl:NamedIndividual>
    


    <!-- http://purl.obolibrary.org/obo/GAZ_00236360 -->

    <owl:NamedIndividual rdf:about="http://purl.obolibrary.org/obo/GAZ_00236360">
        <obo:RO_0001025 rdf:resource="http://purl.obolibrary.org/obo/GAZ_00015452"/>
        <obo:IAO_0000115>An island.</obo:IAO_0000115>
        <oboInOwl:hasOBONamespace>GAZ</oboInOwl:hasOBONamespace>
        <oboInOwl:id>GAZ:00236360</oboInOwl:id>
        <rdfs:label>Sigulu Island</rdfs:label>
    </owl:NamedIndividual>
    


    <!-- http://purl.obolibrary.org/obo/GAZ_00236361 -->

    <owl:NamedIndividual rdf:about="http://purl.obolibrary.org/obo/GAZ_00236361">
        <obo:RO_0001025 rdf:resource="http://purl.obolibrary.org/obo/GAZ_00015452"/>
        <obo:IAO_0000115>An island.</obo:IAO_0000115>
        <oboInOwl:hasOBONamespace>GAZ</oboInOwl:hasOBONamespace>
        <oboInOwl:id>GAZ:00236361</oboInOwl:id>
        <rdfs:label>Seguti Island</rdfs:label>
    </owl:NamedIndividual>
    


    <!-- http://purl.obolibrary.org/obo/GAZ_00236362 -->

    <owl:NamedIndividual rdf:about="http://purl.obolibrary.org/obo/GAZ_00236362">
        <obo:RO_0001025 rdf:resource="http://purl.obolibrary.org/obo/GAZ_00015452"/>
        <obo:IAO_0000115>An island.</obo:IAO_0000115>
        <oboInOwl:hasOBONamespace>GAZ</oboInOwl:hasOBONamespace>
        <oboInOwl:id>GAZ:00236362</oboInOwl:id>
        <rdfs:label>Dagusi Island</rdfs:label>
    </owl:NamedIndividual>
    


    <!-- http://purl.obolibrary.org/obo/GAZ_00236363 -->

    <owl:NamedIndividual rdf:about="http://purl.obolibrary.org/obo/GAZ_00236363">
        <obo:RO_0001025 rdf:resource="http://purl.obolibrary.org/obo/GAZ_00015452"/>
        <obo:IAO_0000115>An island.</obo:IAO_0000115>
        <oboInOwl:hasOBONamespace>GAZ</oboInOwl:hasOBONamespace>
        <oboInOwl:id>GAZ:00236363</oboInOwl:id>
        <rdfs:label>Vumba Island</rdfs:label>
    </owl:NamedIndividual>
    


    <!-- http://purl.obolibrary.org/obo/GAZ_00236364 -->

    <owl:NamedIndividual rdf:about="http://purl.obolibrary.org/obo/GAZ_00236364">
        <obo:RO_0001025 rdf:resource="http://purl.obolibrary.org/obo/GAZ_00015452"/>
        <obo:IAO_0000115>An island.</obo:IAO_0000115>
        <oboInOwl:hasOBONamespace>GAZ</oboInOwl:hasOBONamespace>
        <oboInOwl:id>GAZ:00236364</oboInOwl:id>
        <rdfs:label>Kaza Island</rdfs:label>
    </owl:NamedIndividual>
    


    <!-- http://purl.obolibrary.org/obo/GAZ_00236365 -->

    <owl:NamedIndividual rdf:about="http://purl.obolibrary.org/obo/GAZ_00236365">
        <obo:RO_0001025 rdf:resource="http://purl.obolibrary.org/obo/GAZ_00015452"/>
        <obo:IAO_0000115>An island.</obo:IAO_0000115>
        <oboInOwl:hasOBONamespace>GAZ</oboInOwl:hasOBONamespace>
        <oboInOwl:id>GAZ:00236365</oboInOwl:id>
        <rdfs:label>Nambuga Island</rdfs:label>
    </owl:NamedIndividual>
    


    <!-- http://purl.obolibrary.org/obo/GAZ_00236366 -->

    <owl:NamedIndividual rdf:about="http://purl.obolibrary.org/obo/GAZ_00236366">
        <obo:RO_0001025 rdf:resource="http://purl.obolibrary.org/obo/GAZ_00015452"/>
        <obo:IAO_0000115>An island.</obo:IAO_0000115>
        <oboInOwl:hasOBONamespace>GAZ</oboInOwl:hasOBONamespace>
        <oboInOwl:id>GAZ:00236366</oboInOwl:id>
        <rdfs:label>Simu Island</rdfs:label>
    </owl:NamedIndividual>
    


    <!-- http://purl.obolibrary.org/obo/GAZ_00236597 -->

    <owl:NamedIndividual rdf:about="http://purl.obolibrary.org/obo/GAZ_00236597">
        <obo:RO_0001025 rdf:resource="http://purl.obolibrary.org/obo/GAZ_00040046"/>
        <obo:IAO_0000115>An island.</obo:IAO_0000115>
        <oboInOwl:hasOBONamespace>GAZ</oboInOwl:hasOBONamespace>
        <oboInOwl:id>GAZ:00236597</oboInOwl:id>
        <rdfs:label>Ngamba Island</rdfs:label>
    </owl:NamedIndividual>
    


    <!-- http://purl.obolibrary.org/obo/GAZ_00236598 -->

    <owl:NamedIndividual rdf:about="http://purl.obolibrary.org/obo/GAZ_00236598">
        <obo:RO_0001025 rdf:resource="http://purl.obolibrary.org/obo/GAZ_00040046"/>
        <obo:IAO_0000115>An island.</obo:IAO_0000115>
        <oboInOwl:hasOBONamespace>GAZ</oboInOwl:hasOBONamespace>
        <oboInOwl:id>GAZ:00236598</oboInOwl:id>
        <rdfs:label>Nsadzi Island</rdfs:label>
    </owl:NamedIndividual>
    


    <!-- http://purl.obolibrary.org/obo/GAZ_00236599 -->

    <owl:NamedIndividual rdf:about="http://purl.obolibrary.org/obo/GAZ_00236599">
        <obo:RO_0001025 rdf:resource="http://purl.obolibrary.org/obo/GAZ_00040046"/>
        <obo:IAO_0000115>An island.</obo:IAO_0000115>
        <oboInOwl:hasOBONamespace>GAZ</oboInOwl:hasOBONamespace>
        <oboInOwl:id>GAZ:00236599</oboInOwl:id>
        <rdfs:label>Bulago Island</rdfs:label>
    </owl:NamedIndividual>
    


    <!-- http://purl.obolibrary.org/obo/GAZ_00237137 -->

    <owl:NamedIndividual rdf:about="http://purl.obolibrary.org/obo/GAZ_00237137">
        <obo:IAO_0000115>A wide, 32 km long body of water that links Lake Edward and Lake George, and a dominant feature of Queen Elizabeth National Park.</obo:IAO_0000115>
        <oboInOwl:hasOBONamespace>GAZ</oboInOwl:hasOBONamespace>
        <oboInOwl:id>GAZ:00237137</oboInOwl:id>
        <rdfs:label>Kazinga Channel</rdfs:label>
    </owl:NamedIndividual>
    


    <!-- http://purl.obolibrary.org/obo/GAZ_00237174 -->

    <owl:NamedIndividual rdf:about="http://purl.obolibrary.org/obo/GAZ_00237174">
        <obo:IAO_0000115>A hydroelectric power station across the White Nile near to its source at Lake Victoria in Uganda.</obo:IAO_0000115>
        <oboInOwl:hasOBONamespace>GAZ</oboInOwl:hasOBONamespace>
        <oboInOwl:id>GAZ:00237174</oboInOwl:id>
        <rdfs:label>Nalubaale Power Station</rdfs:label>
    </owl:NamedIndividual>
    


    <!-- http://purl.obolibrary.org/obo/GAZ_00237175 -->

    <owl:NamedIndividual rdf:about="http://purl.obolibrary.org/obo/GAZ_00237175">
        <obo:IAO_0000115>A hydroelectric power station located in Jinja, Jinja District, in eastern central Uganda.</obo:IAO_0000115>
        <oboInOwl:hasOBONamespace>GAZ</oboInOwl:hasOBONamespace>
        <oboInOwl:id>GAZ:00237175</oboInOwl:id>
        <rdfs:label>Kiira Power Station</rdfs:label>
    </owl:NamedIndividual>
    


    <!-- http://purl.obolibrary.org/obo/GAZ_00237176 -->

    <owl:NamedIndividual rdf:about="http://purl.obolibrary.org/obo/GAZ_00237176">
        <obo:IAO_0000115>A hydroelectric power project located at the headwaters of River Nile, about 16 km north of Jinja at the former location of Bujagali Falls.</obo:IAO_0000115>
        <oboInOwl:hasOBONamespace>GAZ</oboInOwl:hasOBONamespace>
        <oboInOwl:id>GAZ:00237176</oboInOwl:id>
        <rdfs:label>Bujagali Power Station</rdfs:label>
    </owl:NamedIndividual>
    


    <!-- http://purl.obolibrary.org/obo/GAZ_00237412 -->

    <owl:NamedIndividual rdf:about="http://purl.obolibrary.org/obo/GAZ_00237412">
        <obo:IAO_0000115>A river of eastern Uganda in eastern Africa. It flows in a southern and south-westerly direction and eventually via the Okere River reaches Lake Kyoga.</obo:IAO_0000115>
        <oboInOwl:hasOBONamespace>GAZ</oboInOwl:hasOBONamespace>
        <oboInOwl:id>GAZ:00237412</oboInOwl:id>
        <rdfs:label>Okot River</rdfs:label>
    </owl:NamedIndividual>
    


    <!-- http://purl.obolibrary.org/obo/GAZ_00237449 -->

    <owl:NamedIndividual rdf:about="http://purl.obolibrary.org/obo/GAZ_00237449">
        <obo:IAO_0000115>A river.</obo:IAO_0000115>
        <oboInOwl:hasOBONamespace>GAZ</oboInOwl:hasOBONamespace>
        <oboInOwl:id>GAZ:00237449</oboInOwl:id>
        <rdfs:label>Lufubu River</rdfs:label>
    </owl:NamedIndividual>
    


    <!-- http://purl.obolibrary.org/obo/GAZ_00240890 -->

    <owl:NamedIndividual rdf:about="http://purl.obolibrary.org/obo/GAZ_00240890">
        <obo:RO_0001025 rdf:resource="http://purl.obolibrary.org/obo/GAZ_00008558"/>
        <obo:IAO_0000115>An island.</obo:IAO_0000115>
        <oboInOwl:hasOBONamespace>GAZ</oboInOwl:hasOBONamespace>
        <oboInOwl:id>GAZ:00240890</oboInOwl:id>
        <rdfs:label>Ile Wahu</rdfs:label>
    </owl:NamedIndividual>
    


    <!-- http://purl.obolibrary.org/obo/GAZ_00240891 -->

    <owl:NamedIndividual rdf:about="http://purl.obolibrary.org/obo/GAZ_00240891">
        <obo:RO_0001025 rdf:resource="http://purl.obolibrary.org/obo/GAZ_00008558"/>
        <obo:IAO_0000115>An island.</obo:IAO_0000115>
        <oboInOwl:hasOBONamespace>GAZ</oboInOwl:hasOBONamespace>
        <oboInOwl:id>GAZ:00240891</oboInOwl:id>
        <rdfs:label>Ile Bugarura</rdfs:label>
    </owl:NamedIndividual>
    


    <!-- http://purl.obolibrary.org/obo/GAZ_00240892 -->

    <owl:NamedIndividual rdf:about="http://purl.obolibrary.org/obo/GAZ_00240892">
        <obo:RO_0001025 rdf:resource="http://purl.obolibrary.org/obo/GAZ_00008558"/>
        <obo:IAO_0000115>An island.</obo:IAO_0000115>
        <oboInOwl:hasOBONamespace>GAZ</oboInOwl:hasOBONamespace>
        <oboInOwl:id>GAZ:00240892</oboInOwl:id>
        <rdfs:label>Ile Gombe</rdfs:label>
    </owl:NamedIndividual>
    


    <!-- http://purl.obolibrary.org/obo/GAZ_00247089 -->

    <owl:NamedIndividual rdf:about="http://purl.obolibrary.org/obo/GAZ_00247089">
        <obo:IAO_0000115>A river. A tributary of the Ruvyironza River.</obo:IAO_0000115>
        <oboInOwl:hasOBONamespace>GAZ</oboInOwl:hasOBONamespace>
        <oboInOwl:id>GAZ:00247089</oboInOwl:id>
        <rdfs:label>Karuzi River</rdfs:label>
    </owl:NamedIndividual>
    


    <!-- http://purl.obolibrary.org/obo/GAZ_00247090 -->

    <owl:NamedIndividual rdf:about="http://purl.obolibrary.org/obo/GAZ_00247090">
        <obo:IAO_0000115>A river. It rises in the far east of Burundi, close to the Tanzanian border, and flows southwestwards, anti-parallel with the Rurubu for 48 km, before turning abruptly northwards to a confluence with the Rurubu.</obo:IAO_0000115>
        <oboInOwl:hasOBONamespace>GAZ</oboInOwl:hasOBONamespace>
        <oboInOwl:id>GAZ:00247090</oboInOwl:id>
        <rdfs:label>Kayongozi River</rdfs:label>
    </owl:NamedIndividual>
    


    <!-- http://purl.obolibrary.org/obo/GAZ_00247094 -->

    <owl:NamedIndividual rdf:about="http://purl.obolibrary.org/obo/GAZ_00247094">
        <obo:IAO_0000115>A river that flows into Lake Tanganyika in the south of Burundi.</obo:IAO_0000115>
        <oboInOwl:hasOBONamespace>GAZ</oboInOwl:hasOBONamespace>
        <oboInOwl:id>GAZ:00247094</oboInOwl:id>
        <rdfs:label>Mugwezi River</rdfs:label>
    </owl:NamedIndividual>
    


    <!-- http://purl.obolibrary.org/obo/GAZ_00247095 -->

    <owl:NamedIndividual rdf:about="http://purl.obolibrary.org/obo/GAZ_00247095">
        <obo:IAO_0000115>A river that flows into Lake Tanganyika in the south of Burundi.</obo:IAO_0000115>
        <oboInOwl:hasOBONamespace>GAZ</oboInOwl:hasOBONamespace>
        <oboInOwl:id>GAZ:00247095</oboInOwl:id>
        <rdfs:label>Luaba River</rdfs:label>
    </owl:NamedIndividual>
    


    <!-- http://purl.obolibrary.org/obo/GAZ_00248108 -->

    <owl:NamedIndividual rdf:about="http://purl.obolibrary.org/obo/GAZ_00248108">
        <obo:RO_0001025 rdf:resource="http://purl.obolibrary.org/obo/GAZ_10000775"/>
        <obo:IAO_0000115>A lake.</obo:IAO_0000115>
        <oboInOwl:hasOBONamespace>GAZ</oboInOwl:hasOBONamespace>
        <oboInOwl:id>GAZ:00248108</oboInOwl:id>
        <rdfs:label>Lake Mandalum</rdfs:label>
    </owl:NamedIndividual>
    


    <!-- http://purl.obolibrary.org/obo/GAZ_00248109 -->

    <owl:NamedIndividual rdf:about="http://purl.obolibrary.org/obo/GAZ_00248109">
        <obo:RO_0001025 rdf:resource="http://purl.obolibrary.org/obo/GAZ_10000775"/>
        <obo:IAO_0000115>A protected area.</obo:IAO_0000115>
        <oboInOwl:hasOBONamespace>GAZ</oboInOwl:hasOBONamespace>
        <oboInOwl:id>GAZ:00248109</oboInOwl:id>
        <rdfs:label>Yob Wildlife Reserve</rdfs:label>
    </owl:NamedIndividual>
    


    <!-- http://purl.obolibrary.org/obo/GAZ_00248110 -->

    <owl:NamedIndividual rdf:about="http://purl.obolibrary.org/obo/GAZ_00248110">
        <obo:RO_0001025 rdf:resource="http://purl.obolibrary.org/obo/GAZ_10000775"/>
        <obo:IAO_0000115>A protected area.</obo:IAO_0000115>
        <oboInOwl:hasOBONamespace>GAZ</oboInOwl:hasOBONamespace>
        <oboInOwl:id>GAZ:00248110</oboInOwl:id>
        <rdfs:label>Nafka Wildlife Reserve</rdfs:label>
    </owl:NamedIndividual>
    


    <!-- http://purl.obolibrary.org/obo/GAZ_00248111 -->

    <owl:NamedIndividual rdf:about="http://purl.obolibrary.org/obo/GAZ_00248111">
        <obo:RO_0001025 rdf:resource="http://purl.obolibrary.org/obo/GAZ_10000775"/>
        <obo:IAO_0000115>A bay.</obo:IAO_0000115>
        <oboInOwl:hasOBONamespace>GAZ</oboInOwl:hasOBONamespace>
        <oboInOwl:id>GAZ:00248111</oboInOwl:id>
        <rdfs:label>Mersa Mubarec</rdfs:label>
    </owl:NamedIndividual>
    


    <!-- http://purl.obolibrary.org/obo/GAZ_00248112 -->

    <owl:NamedIndividual rdf:about="http://purl.obolibrary.org/obo/GAZ_00248112">
        <obo:RO_0001025 rdf:resource="http://purl.obolibrary.org/obo/GAZ_10000775"/>
        <obo:IAO_0000115>An inlet.</obo:IAO_0000115>
        <oboInOwl:hasOBONamespace>GAZ</oboInOwl:hasOBONamespace>
        <oboInOwl:id>GAZ:00248112</oboInOwl:id>
        <rdfs:label>Mersa Deresa</rdfs:label>
    </owl:NamedIndividual>
    


    <!-- http://purl.obolibrary.org/obo/GAZ_00248113 -->

    <owl:NamedIndividual rdf:about="http://purl.obolibrary.org/obo/GAZ_00248113">
        <rdf:type rdf:resource="http://purl.obolibrary.org/obo/ENVO_00000004"/>
        <obo:RO_0001025 rdf:resource="http://purl.obolibrary.org/obo/GAZ_00000776"/>
        <obo:IAO_0000115>A district of the Southern Region of Eritrea.</obo:IAO_0000115>
        <oboInOwl:hasOBONamespace>GAZ</oboInOwl:hasOBONamespace>
        <oboInOwl:id>GAZ:00248113</oboInOwl:id>
        <rdfs:label>Tserona District</rdfs:label>
    </owl:NamedIndividual>
    


    <!-- http://purl.obolibrary.org/obo/GAZ_00248114 -->

    <owl:NamedIndividual rdf:about="http://purl.obolibrary.org/obo/GAZ_00248114">
        <rdf:type rdf:resource="http://purl.obolibrary.org/obo/ENVO_00000004"/>
        <obo:RO_0001025 rdf:resource="http://purl.obolibrary.org/obo/GAZ_00000776"/>
        <obo:IAO_0000115>A district of the Southern Region of Eritrea.</obo:IAO_0000115>
        <oboInOwl:hasOBONamespace>GAZ</oboInOwl:hasOBONamespace>
        <oboInOwl:id>GAZ:00248114</oboInOwl:id>
        <rdfs:label>Hadidia District</rdfs:label>
    </owl:NamedIndividual>
    


    <!-- http://purl.obolibrary.org/obo/GAZ_00248115 -->

    <owl:NamedIndividual rdf:about="http://purl.obolibrary.org/obo/GAZ_00248115">
        <rdf:type rdf:resource="http://purl.obolibrary.org/obo/ENVO_00000004"/>
        <obo:RO_0001025 rdf:resource="http://purl.obolibrary.org/obo/GAZ_00000776"/>
        <obo:IAO_0000115>A district of the Southern Region of Eritrea.</obo:IAO_0000115>
        <oboInOwl:hasOBONamespace>GAZ</oboInOwl:hasOBONamespace>
        <oboInOwl:id>GAZ:00248115</oboInOwl:id>
        <rdfs:label>Tera-Emni District</rdfs:label>
    </owl:NamedIndividual>
    


    <!-- http://purl.obolibrary.org/obo/GAZ_00248116 -->

    <owl:NamedIndividual rdf:about="http://purl.obolibrary.org/obo/GAZ_00248116">
        <obo:RO_0001025 rdf:resource="http://purl.obolibrary.org/obo/GAZ_00000777"/>
        <obo:IAO_0000115>A populated place. A port city in the Southern Red Sea Region of Eritrea on the west coast of the Red Sea.</obo:IAO_0000115>
        <oboInOwl:hasOBONamespace>GAZ</oboInOwl:hasOBONamespace>
        <oboInOwl:id>GAZ:00248116</oboInOwl:id>
        <rdfs:label>Assab</rdfs:label>
    </owl:NamedIndividual>
    


    <!-- http://purl.obolibrary.org/obo/GAZ_00248117 -->

    <owl:NamedIndividual rdf:about="http://purl.obolibrary.org/obo/GAZ_00248117">
        <obo:RO_0001025 rdf:resource="http://purl.obolibrary.org/obo/GAZ_00000777"/>
        <obo:IAO_0000115>A bay.</obo:IAO_0000115>
        <oboInOwl:hasOBONamespace>GAZ</oboInOwl:hasOBONamespace>
        <oboInOwl:id>GAZ:00248117</oboInOwl:id>
        <rdfs:label>Assab Bahir Selat&apos;e</rdfs:label>
    </owl:NamedIndividual>
    


    <!-- http://purl.obolibrary.org/obo/GAZ_00248118 -->

    <owl:NamedIndividual rdf:about="http://purl.obolibrary.org/obo/GAZ_00248118">
        <obo:RO_0001025 rdf:resource="http://purl.obolibrary.org/obo/GAZ_00248117"/>
        <obo:IAO_0000115>An island.</obo:IAO_0000115>
        <oboInOwl:hasOBONamespace>GAZ</oboInOwl:hasOBONamespace>
        <oboInOwl:id>GAZ:00248118</oboInOwl:id>
        <rdfs:label>Fatuma Deset</rdfs:label>
    </owl:NamedIndividual>
    


    <!-- http://purl.obolibrary.org/obo/GAZ_00248119 -->

    <owl:NamedIndividual rdf:about="http://purl.obolibrary.org/obo/GAZ_00248119">
        <obo:RO_0001025 rdf:resource="http://purl.obolibrary.org/obo/GAZ_00052532"/>
        <obo:IAO_0000115>A freshwater lake.</obo:IAO_0000115>
        <oboInOwl:hasOBONamespace>GAZ</oboInOwl:hasOBONamespace>
        <oboInOwl:id>GAZ:00248119</oboInOwl:id>
        <rdfs:label>Garba Gurastch Lake</rdfs:label>
    </owl:NamedIndividual>
    


    <!-- http://purl.obolibrary.org/obo/GAZ_00248120 -->

    <owl:NamedIndividual rdf:about="http://purl.obolibrary.org/obo/GAZ_00248120">
        <obo:RO_0001025 rdf:resource="http://purl.obolibrary.org/obo/GAZ_00052532"/>
        <obo:IAO_0000115>A freshwater lake.</obo:IAO_0000115>
        <oboInOwl:hasOBONamespace>GAZ</oboInOwl:hasOBONamespace>
        <oboInOwl:id>GAZ:00248120</oboInOwl:id>
        <rdfs:label>Hora Orgona Lake</rdfs:label>
    </owl:NamedIndividual>
    


    <!-- http://purl.obolibrary.org/obo/GAZ_00248126 -->

    <owl:NamedIndividual rdf:about="http://purl.obolibrary.org/obo/GAZ_00248126">
        <rdf:type rdf:resource="http://purl.obolibrary.org/obo/ENVO_00000309"/>
        <obo:RO_0001025 rdf:resource="http://purl.obolibrary.org/obo/GAZ_00000007"/>
        <obo:IAO_0000115>A pan.</obo:IAO_0000115>
        <oboInOwl:hasOBONamespace>GAZ</oboInOwl:hasOBONamespace>
        <oboInOwl:id>GAZ:00248126</oboInOwl:id>
        <rdfs:label>Ch&apos;ew Bahir</rdfs:label>
    </owl:NamedIndividual>
    


    <!-- http://purl.obolibrary.org/obo/GAZ_00248136 -->

    <owl:NamedIndividual rdf:about="http://purl.obolibrary.org/obo/GAZ_00248136">
        <obo:RO_0001025 rdf:resource="http://purl.obolibrary.org/obo/GAZ_00051205"/>
        <obo:IAO_0000115>A saline lake.</obo:IAO_0000115>
        <oboInOwl:hasOBONamespace>GAZ</oboInOwl:hasOBONamespace>
        <oboInOwl:id>GAZ:00248136</oboInOwl:id>
        <rdfs:label>Lake Asale</rdfs:label>
    </owl:NamedIndividual>
    


    <!-- http://purl.obolibrary.org/obo/GAZ_00248137 -->

    <owl:NamedIndividual rdf:about="http://purl.obolibrary.org/obo/GAZ_00248137">
        <obo:IAO_0000115>A reservoir in Ethiopia. Constructed 1960.</obo:IAO_0000115>
        <oboInOwl:hasOBONamespace>GAZ</oboInOwl:hasOBONamespace>
        <oboInOwl:id>GAZ:00248137</oboInOwl:id>
        <rdfs:label>Zula Lake</rdfs:label>
    </owl:NamedIndividual>
    


    <!-- http://purl.obolibrary.org/obo/GAZ_00251586 -->

    <owl:NamedIndividual rdf:about="http://purl.obolibrary.org/obo/GAZ_00251586">
        <obo:IAO_0000115>A river that rises in the hills southwest of Irbid city and drains west into the Jordan Valley, entering the Jordan River about 20 km south of Lake Tiberias.</obo:IAO_0000115>
        <oboInOwl:hasOBONamespace>GAZ</oboInOwl:hasOBONamespace>
        <oboInOwl:id>GAZ:00251586</oboInOwl:id>
        <rdfs:label>Wadi Ziglab</rdfs:label>
    </owl:NamedIndividual>
    


    <!-- http://purl.obolibrary.org/obo/GAZ_00251587 -->

    <owl:NamedIndividual rdf:about="http://purl.obolibrary.org/obo/GAZ_00251587">
        <obo:IAO_0000115>A dam. Located about 15 km south-southwest of Ajlun.</obo:IAO_0000115>
        <oboInOwl:hasOBONamespace>GAZ</oboInOwl:hasOBONamespace>
        <oboInOwl:id>GAZ:00251587</oboInOwl:id>
        <rdfs:label>KingTalal Dam</rdfs:label>
    </owl:NamedIndividual>
    


    <!-- http://purl.obolibrary.org/obo/GAZ_00251592 -->

    <owl:NamedIndividual rdf:about="http://purl.obolibrary.org/obo/GAZ_00251592">
        <obo:IAO_0000115>A dam.</obo:IAO_0000115>
        <oboInOwl:hasOBONamespace>GAZ</oboInOwl:hasOBONamespace>
        <oboInOwl:id>GAZ:00251592</oboInOwl:id>
        <rdfs:label>Kafrein Dam</rdfs:label>
    </owl:NamedIndividual>
    


    <!-- http://purl.obolibrary.org/obo/GAZ_00251593 -->

    <owl:NamedIndividual rdf:about="http://purl.obolibrary.org/obo/GAZ_00251593">
        <obo:IAO_0000115>A dam.</obo:IAO_0000115>
        <oboInOwl:hasOBONamespace>GAZ</oboInOwl:hasOBONamespace>
        <oboInOwl:id>GAZ:00251593</oboInOwl:id>
        <rdfs:label>Shu&apos;eib Dam</rdfs:label>
    </owl:NamedIndividual>
    


    <!-- http://purl.obolibrary.org/obo/GAZ_00251594 -->

    <owl:NamedIndividual rdf:about="http://purl.obolibrary.org/obo/GAZ_00251594">
        <obo:RO_0001025 rdf:resource="http://purl.obolibrary.org/obo/GAZ_00044915"/>
        <obo:IAO_0000115>A saline lake.</obo:IAO_0000115>
        <oboInOwl:hasOBONamespace>GAZ</oboInOwl:hasOBONamespace>
        <oboInOwl:id>GAZ:00251594</oboInOwl:id>
        <rdfs:label>Kibed Pool</rdfs:label>
    </owl:NamedIndividual>
    


    <!-- http://purl.obolibrary.org/obo/GAZ_00251595 -->

    <owl:NamedIndividual rdf:about="http://purl.obolibrary.org/obo/GAZ_00251595">
        <obo:IAO_0000115>A wadi. It enters Wadi Mujib from the north only a few km from the shores of the Dead Sea.</obo:IAO_0000115>
        <oboInOwl:hasOBONamespace>GAZ</oboInOwl:hasOBONamespace>
        <oboInOwl:id>GAZ:00251595</oboInOwl:id>
        <rdfs:label>Wadi Hidan</rdfs:label>
    </owl:NamedIndividual>
    


    <!-- http://purl.obolibrary.org/obo/GAZ_00251642 -->

    <owl:NamedIndividual rdf:about="http://purl.obolibrary.org/obo/GAZ_00251642">
        <obo:RO_0001025 rdf:resource="http://purl.obolibrary.org/obo/GAZ_00041537"/>
        <obo:IAO_0000115>A part of Lake Naivasha. It becomes a discrete, but contiguous, basin at low water.</obo:IAO_0000115>
        <oboInOwl:hasOBONamespace>GAZ</oboInOwl:hasOBONamespace>
        <oboInOwl:id>GAZ:00251642</oboInOwl:id>
        <rdfs:label>Lake Oloidien</rdfs:label>
    </owl:NamedIndividual>
    


    <!-- http://purl.obolibrary.org/obo/GAZ_00251652 -->

    <owl:NamedIndividual rdf:about="http://purl.obolibrary.org/obo/GAZ_00251652">
        <obo:RO_0001025 rdf:resource="http://purl.obolibrary.org/obo/GAZ_00000007"/>
        <obo:IAO_0000115>A lake. It is situated on the Nyandarua Plateau at the foot of the Aberdare Mountains.</obo:IAO_0000115>
        <oboInOwl:hasOBONamespace>GAZ</oboInOwl:hasOBONamespace>
        <oboInOwl:id>GAZ:00251652</oboInOwl:id>
        <rdfs:label>Lake Ilpolosat</rdfs:label>
    </owl:NamedIndividual>
    


    <!-- http://purl.obolibrary.org/obo/GAZ_00251653 -->

    <owl:NamedIndividual rdf:about="http://purl.obolibrary.org/obo/GAZ_00251653">
        <obo:IAO_0000115>A river.</obo:IAO_0000115>
        <oboInOwl:hasOBONamespace>GAZ</oboInOwl:hasOBONamespace>
        <oboInOwl:id>GAZ:00251653</oboInOwl:id>
        <rdfs:label>Malewa River</rdfs:label>
    </owl:NamedIndividual>
    


    <!-- http://purl.obolibrary.org/obo/GAZ_00251816 -->

    <owl:NamedIndividual rdf:about="http://purl.obolibrary.org/obo/GAZ_00251816">
        <obo:RO_0001025 rdf:resource="http://purl.obolibrary.org/obo/GAZ_00044906"/>
        <obo:IAO_0000115>A wetland. Located in the western Beka&apos;a Valley south of the main Beirut to Damascus highway, 10 km south-southwest of Qabb Elias town and about 35 km southeast of Beirut.</obo:IAO_0000115>
        <oboInOwl:hasOBONamespace>GAZ</oboInOwl:hasOBONamespace>
        <oboInOwl:id>GAZ:00251816</oboInOwl:id>
        <rdfs:label>Ainmiq Swamp</rdfs:label>
    </owl:NamedIndividual>
    


    <!-- http://purl.obolibrary.org/obo/GAZ_00251903 -->

    <owl:NamedIndividual rdf:about="http://purl.obolibrary.org/obo/GAZ_00251903">
        <obo:IAO_0000115>A widening of the Shire River?</obo:IAO_0000115>
        <oboInOwl:hasOBONamespace>GAZ</oboInOwl:hasOBONamespace>
        <oboInOwl:id>GAZ:00251903</oboInOwl:id>
        <rdfs:label>Bangula Lagoon</rdfs:label>
    </owl:NamedIndividual>
    


    <!-- http://purl.obolibrary.org/obo/GAZ_00251905 -->

    <owl:NamedIndividual rdf:about="http://purl.obolibrary.org/obo/GAZ_00251905">
        <obo:RO_0001025 rdf:resource="http://purl.obolibrary.org/obo/GAZ_00041528"/>
        <obo:IAO_0000115>An island.</obo:IAO_0000115>
        <oboInOwl:hasOBONamespace>GAZ</oboInOwl:hasOBONamespace>
        <oboInOwl:id>GAZ:00251905</oboInOwl:id>
        <rdfs:label>Nchisi Island</rdfs:label>
    </owl:NamedIndividual>
    


    <!-- http://purl.obolibrary.org/obo/GAZ_00255602 -->

    <owl:NamedIndividual rdf:about="http://purl.obolibrary.org/obo/GAZ_00255602">
        <obo:IAO_0000115>A river that carries the overspill from Lake Muhazi.</obo:IAO_0000115>
        <oboInOwl:hasOBONamespace>GAZ</oboInOwl:hasOBONamespace>
        <oboInOwl:id>GAZ:00255602</oboInOwl:id>
        <rdfs:label>Nyabugogo River</rdfs:label>
    </owl:NamedIndividual>
    


    <!-- http://purl.obolibrary.org/obo/GAZ_00256741 -->

    <owl:NamedIndividual rdf:about="http://purl.obolibrary.org/obo/GAZ_00256741">
        <obo:IAO_0000115>A river.</obo:IAO_0000115>
        <oboInOwl:hasOBONamespace>GAZ</oboInOwl:hasOBONamespace>
        <oboInOwl:id>GAZ:00256741</oboInOwl:id>
        <rdfs:label>Ziuwe River</rdfs:label>
    </owl:NamedIndividual>
    


    <!-- http://purl.obolibrary.org/obo/GAZ_00256743 -->

    <owl:NamedIndividual rdf:about="http://purl.obolibrary.org/obo/GAZ_00256743">
        <obo:RO_0001025 rdf:resource="http://purl.obolibrary.org/obo/GAZ_00256741"/>
        <obo:IAO_0000115>A lake.</obo:IAO_0000115>
        <oboInOwl:hasOBONamespace>GAZ</oboInOwl:hasOBONamespace>
        <oboInOwl:id>GAZ:00256743</oboInOwl:id>
        <rdfs:label>Lake Sagara</rdfs:label>
    </owl:NamedIndividual>
    


    <!-- http://purl.obolibrary.org/obo/GAZ_00260236 -->

    <owl:NamedIndividual rdf:about="http://purl.obolibrary.org/obo/GAZ_00260236">
        <obo:RO_0001025 rdf:resource="http://purl.obolibrary.org/obo/GAZ_00015452"/>
        <obo:IAO_0000115>An island. S of Vumba Island.</obo:IAO_0000115>
        <oboInOwl:hasOBONamespace>GAZ</oboInOwl:hasOBONamespace>
        <oboInOwl:id>GAZ:00260236</oboInOwl:id>
        <rdfs:label>Sagitu Island</rdfs:label>
    </owl:NamedIndividual>
    


    <!-- http://purl.obolibrary.org/obo/GAZ_00260237 -->

    <owl:NamedIndividual rdf:about="http://purl.obolibrary.org/obo/GAZ_00260237">
        <obo:RO_0001025 rdf:resource="http://purl.obolibrary.org/obo/GAZ_00015452"/>
        <obo:IAO_0000115>A bay.</obo:IAO_0000115>
        <oboInOwl:hasOBONamespace>GAZ</oboInOwl:hasOBONamespace>
        <oboInOwl:id>GAZ:00260237</oboInOwl:id>
        <rdfs:label>Sango Bay</rdfs:label>
    </owl:NamedIndividual>
    


    <!-- http://purl.obolibrary.org/obo/GAZ_00260238 -->

    <owl:NamedIndividual rdf:about="http://purl.obolibrary.org/obo/GAZ_00260238">
        <obo:RO_0001025 rdf:resource="http://purl.obolibrary.org/obo/GAZ_00015452"/>
        <obo:IAO_0000115>A channel N of Bugala Island.</obo:IAO_0000115>
        <oboInOwl:hasOBONamespace>GAZ</oboInOwl:hasOBONamespace>
        <oboInOwl:id>GAZ:00260238</oboInOwl:id>
        <rdfs:label>Salisbury Channel</rdfs:label>
    </owl:NamedIndividual>
    


    <!-- http://purl.obolibrary.org/obo/GAZ_00260292 -->

    <owl:NamedIndividual rdf:about="http://purl.obolibrary.org/obo/GAZ_00260292">
        <rdf:type rdf:resource="http://purl.obolibrary.org/obo/ENVO_00000475"/>
        <obo:RO_0001025 rdf:resource="http://purl.obolibrary.org/obo/GAZ_00058791"/>
        <obo:IAO_0000115>An arm of Lake Kyoga.</obo:IAO_0000115>
        <oboInOwl:hasOBONamespace>GAZ</oboInOwl:hasOBONamespace>
        <oboInOwl:id>GAZ:00260292</oboInOwl:id>
        <rdfs:label>Mpologoma Arm</rdfs:label>
    </owl:NamedIndividual>
    


    <!-- http://purl.obolibrary.org/obo/GAZ_00260963 -->

    <owl:NamedIndividual rdf:about="http://purl.obolibrary.org/obo/GAZ_00260963">
        <obo:RO_0001025 rdf:resource="http://purl.obolibrary.org/obo/GAZ_00041530"/>
        <obo:IAO_0000115>An island.</obo:IAO_0000115>
        <oboInOwl:hasOBONamespace>GAZ</oboInOwl:hasOBONamespace>
        <oboInOwl:id>GAZ:00260963</oboInOwl:id>
        <rdfs:label>N&apos;Kole Island</rdfs:label>
    </owl:NamedIndividual>
    


    <!-- http://purl.obolibrary.org/obo/GAZ_00260964 -->

    <owl:NamedIndividual rdf:about="http://purl.obolibrary.org/obo/GAZ_00260964">
        <obo:RO_0001025 rdf:resource="http://purl.obolibrary.org/obo/GAZ_00058782"/>
        <obo:IAO_0000115>A lake lagoon in Zambia. It is in the Luapula River swamps south of Lake Mweru, in the Luapula Province of Zambia.</obo:IAO_0000115>
        <oboInOwl:hasOBONamespace>GAZ</oboInOwl:hasOBONamespace>
        <oboInOwl:id>GAZ:00260964</oboInOwl:id>
        <rdfs:label>Pembe Lagoon</rdfs:label>
    </owl:NamedIndividual>
    


    <!-- http://purl.obolibrary.org/obo/GAZ_00260965 -->

    <owl:NamedIndividual rdf:about="http://purl.obolibrary.org/obo/GAZ_00260965">
        <obo:RO_0001025 rdf:resource="http://purl.obolibrary.org/obo/GAZ_00058782"/>
        <obo:IAO_0000115>A lake on the Luapula Floodplain.</obo:IAO_0000115>
        <oboInOwl:hasOBONamespace>GAZ</oboInOwl:hasOBONamespace>
        <oboInOwl:id>GAZ:00260965</oboInOwl:id>
        <rdfs:label>Lake Kuswa</rdfs:label>
    </owl:NamedIndividual>
    


    <!-- http://purl.obolibrary.org/obo/GAZ_00260966 -->

    <owl:NamedIndividual rdf:about="http://purl.obolibrary.org/obo/GAZ_00260966">
        <obo:RO_0001025 rdf:resource="http://purl.obolibrary.org/obo/GAZ_00058782"/>
        <obo:IAO_0000115>A lake on the Luapula Floodplain.</obo:IAO_0000115>
        <oboInOwl:hasOBONamespace>GAZ</oboInOwl:hasOBONamespace>
        <oboInOwl:id>GAZ:00260966</oboInOwl:id>
        <rdfs:label>Lake Kitshomponshi</rdfs:label>
    </owl:NamedIndividual>
    


    <!-- http://purl.obolibrary.org/obo/GAZ_00260967 -->

    <owl:NamedIndividual rdf:about="http://purl.obolibrary.org/obo/GAZ_00260967">
        <obo:RO_0001025 rdf:resource="http://purl.obolibrary.org/obo/GAZ_00058782"/>
        <obo:IAO_0000115>A lake on the Luapula Floodplain.</obo:IAO_0000115>
        <oboInOwl:hasOBONamespace>GAZ</oboInOwl:hasOBONamespace>
        <oboInOwl:id>GAZ:00260967</oboInOwl:id>
        <rdfs:label>Lake Kifukula</rdfs:label>
    </owl:NamedIndividual>
    


    <!-- http://purl.obolibrary.org/obo/GAZ_00260968 -->

    <owl:NamedIndividual rdf:about="http://purl.obolibrary.org/obo/GAZ_00260968">
        <obo:RO_0001025 rdf:resource="http://purl.obolibrary.org/obo/GAZ_00058782"/>
        <obo:IAO_0000115>A lake on the Luapula Floodplain.</obo:IAO_0000115>
        <oboInOwl:hasOBONamespace>GAZ</oboInOwl:hasOBONamespace>
        <oboInOwl:id>GAZ:00260968</oboInOwl:id>
        <rdfs:label>Lake Kainsa</rdfs:label>
    </owl:NamedIndividual>
    


    <!-- http://purl.obolibrary.org/obo/GAZ_00260969 -->

    <owl:NamedIndividual rdf:about="http://purl.obolibrary.org/obo/GAZ_00260969">
        <obo:RO_0001025 rdf:resource="http://purl.obolibrary.org/obo/GAZ_00058782"/>
        <obo:IAO_0000115>A lake on the Luapula Floodplain.</obo:IAO_0000115>
        <oboInOwl:hasOBONamespace>GAZ</oboInOwl:hasOBONamespace>
        <oboInOwl:id>GAZ:00260969</oboInOwl:id>
        <rdfs:label>Lake Kinseneka</rdfs:label>
    </owl:NamedIndividual>
    


    <!-- http://purl.obolibrary.org/obo/GAZ_00260970 -->

    <owl:NamedIndividual rdf:about="http://purl.obolibrary.org/obo/GAZ_00260970">
        <obo:RO_0001025 rdf:resource="http://purl.obolibrary.org/obo/GAZ_00041532"/>
        <obo:IAO_0000115>An island.</obo:IAO_0000115>
        <oboInOwl:hasOBONamespace>GAZ</oboInOwl:hasOBONamespace>
        <oboInOwl:id>GAZ:00260970</oboInOwl:id>
        <rdfs:label>Katima Island</rdfs:label>
    </owl:NamedIndividual>
    


    <!-- http://purl.obolibrary.org/obo/GAZ_00281370 -->

    <owl:NamedIndividual rdf:about="http://purl.obolibrary.org/obo/GAZ_00281370">
        <obo:RO_0001025 rdf:resource="http://purl.obolibrary.org/obo/GAZ_10000775"/>
        <obo:IAO_0000115>An archeological site in the Northern Red Sea region of Eritrea, about 30 miles south of Massawa.</obo:IAO_0000115>
        <oboInOwl:hasOBONamespace>GAZ</oboInOwl:hasOBONamespace>
        <oboInOwl:id>GAZ:00281370</oboInOwl:id>
        <rdfs:label>Adulis</rdfs:label>
    </owl:NamedIndividual>
    


    <!-- http://purl.obolibrary.org/obo/GAZ_00281371 -->

    <owl:NamedIndividual rdf:about="http://purl.obolibrary.org/obo/GAZ_00281371">
        <obo:RO_0001025 rdf:resource="http://purl.obolibrary.org/obo/GAZ_00000776"/>
        <obo:IAO_0000115>An archeological site in Eritrea (a few kilometers south of Senafe) and was a major Aksumite and Pre-Aksumite city.</obo:IAO_0000115>
        <oboInOwl:hasOBONamespace>GAZ</oboInOwl:hasOBONamespace>
        <oboInOwl:id>GAZ:00281371</oboInOwl:id>
        <rdfs:label>Matara</rdfs:label>
    </owl:NamedIndividual>
    


    <!-- http://purl.obolibrary.org/obo/GAZ_00281372 -->

    <owl:NamedIndividual rdf:about="http://purl.obolibrary.org/obo/GAZ_00281372">
        <obo:RO_0001025 rdf:resource="http://purl.obolibrary.org/obo/GAZ_00000776"/>
        <obo:IAO_0000115>An archeological site. A pre-Aksumite city that thrived during the Aksumite period.</obo:IAO_0000115>
        <oboInOwl:hasOBONamespace>GAZ</oboInOwl:hasOBONamespace>
        <oboInOwl:id>GAZ:00281372</oboInOwl:id>
        <rdfs:label>Qohaito</rdfs:label>
    </owl:NamedIndividual>
    


    <!-- http://purl.obolibrary.org/obo/GAZ_00281432 -->

    <owl:NamedIndividual rdf:about="http://purl.obolibrary.org/obo/GAZ_00281432">
        <obo:RO_0001025 rdf:resource="http://purl.obolibrary.org/obo/GAZ_00124306"/>
        <obo:IAO_0000115>An archeological site. A Late Stone Age site in Mau Escarpment of Kenya.</obo:IAO_0000115>
        <oboInOwl:hasOBONamespace>GAZ</oboInOwl:hasOBONamespace>
        <oboInOwl:id>GAZ:00281432</oboInOwl:id>
        <rdfs:label>Enkapune Ya Muto</rdfs:label>
    </owl:NamedIndividual>
    


    <!-- http://purl.obolibrary.org/obo/GAZ_00281451 -->

    <owl:NamedIndividual rdf:about="http://purl.obolibrary.org/obo/GAZ_00281451">
        <obo:IAO_0000115>A single drop waterfall on the border of Zambia and Tanzania at the southeast end of Lake Tanganyika.</obo:IAO_0000115>
        <oboInOwl:hasOBONamespace>GAZ</oboInOwl:hasOBONamespace>
        <oboInOwl:id>GAZ:00281451</oboInOwl:id>
        <rdfs:label>Kalambo Falls</rdfs:label>
    </owl:NamedIndividual>
    


    <!-- http://purl.obolibrary.org/obo/GAZ_10000775 -->

    <owl:NamedIndividual rdf:about="http://purl.obolibrary.org/obo/GAZ_10000775"/>
    


    <!-- 
    ///////////////////////////////////////////////////////////////////////////////////////
    //
    // Annotations
    //
    ///////////////////////////////////////////////////////////////////////////////////////
     -->

    <rdf:Description rdf:about="http://purl.obolibrary.org/obo/GAZ_00000771">
        <rdfs:label>Region (Eritrea)</rdfs:label>
        <oboInOwl:hasOBONamespace>GAZ</oboInOwl:hasOBONamespace>
        <oboInOwl:id>GAZ:00000771</oboInOwl:id>
    </rdf:Description>
    <rdf:Description rdf:about="http://purl.obolibrary.org/obo/GAZ_00000772">
        <obo:IAO_0000115>An inland region of Eritrea, in the west of the country. Its capital is Keren.</obo:IAO_0000115>
        <rdfs:label>Anseba Region</rdfs:label>
        <oboInOwl:hasOBONamespace>GAZ</oboInOwl:hasOBONamespace>
        <oboInOwl:id>GAZ:00000772</oboInOwl:id>
    </rdf:Description>
    <rdf:Description rdf:about="http://purl.obolibrary.org/obo/GAZ_00000773">
        <obo:IAO_0000115>One of the six regions of Eritrea. It is the smallest region in area, and contains the major city and national capital, Asmara. The region is inland, and borders Anseba to the north-west, Northern Red Sea region to the north-east, Southern region to the south, and Gash-Barka to the west.</obo:IAO_0000115>
        <oboInOwl:id>GAZ:00000773</oboInOwl:id>
        <rdfs:label>Central Region</rdfs:label>
        <oboInOwl:hasOBONamespace>GAZ</oboInOwl:hasOBONamespace>
    </rdf:Description>
    <rdf:Description rdf:about="http://purl.obolibrary.org/obo/GAZ_00000774">
        <rdfs:label>Gash-Barka Region</rdfs:label>
        <oboInOwl:id>GAZ:00000774</oboInOwl:id>
        <obo:IAO_0000115>One of the six regions of Eritrea. It is situated in the south-west of the country, bordering the Anseba region to the north, and the Central and Southern regions to the east; the county of Sudan lies to the west and Ethiopia to the south.</obo:IAO_0000115>
        <oboInOwl:hasOBONamespace>GAZ</oboInOwl:hasOBONamespace>
    </rdf:Description>
    <rdf:Description rdf:about="http://purl.obolibrary.org/obo/GAZ_00000776">
        <oboInOwl:hasOBONamespace>GAZ</oboInOwl:hasOBONamespace>
        <oboInOwl:id>GAZ:00000776</oboInOwl:id>
        <rdfs:label>Southern Region</rdfs:label>
        <obo:IAO_0000115>A region of Eritrea. It lies along a portion of the national border with Ethiopia. It shares its western border with the region of Gash-Barka, its north with Maakel (central) and its eastern with the Northern Red Sea region.</obo:IAO_0000115>
    </rdf:Description>
    <rdf:Description rdf:about="http://purl.obolibrary.org/obo/GAZ_00000777">
        <obo:IAO_0000115>One of the six main regions of Eritrea. It lies along the southern half of the Red Sea, and contains the coastal city of Asseb. It borders the Northern Red Sea region.</obo:IAO_0000115>
        <oboInOwl:hasOBONamespace>GAZ</oboInOwl:hasOBONamespace>
        <rdfs:label>Southern Red Sea Region</rdfs:label>
        <oboInOwl:id>GAZ:00000777</oboInOwl:id>
    </rdf:Description>
    <rdf:Description rdf:about="http://purl.obolibrary.org/obo/GAZ_10000775">
        <oboInOwl:hasOBONamespace>GAZ</oboInOwl:hasOBONamespace>
        <oboInOwl:id>GAZ:10000775</oboInOwl:id>
        <obo:IAO_0000115>A region of Eritrea. It lies along the northern three quarters of the Red Sea, and includes the Dahlak Archipelago and the coastal city of Massawa. The region borders the Anseba, Central and Southern regions to the west, and the Southern Red Sea region to the east.</obo:IAO_0000115>
        <rdfs:label>Northern Red Sea Region</rdfs:label>
    </rdf:Description>
</rdf:RDF>



<!-- Generated by the OWL API (version 4.5.6) https://github.com/owlcs/owlapi -->

