<?xml version="1.0"?>
<rdf:RDF xmlns="http://purl.obolibrary.org/obo/gaz/subsets/countries/Ethiopia.owl#"
     xml:base="http://purl.obolibrary.org/obo/gaz/subsets/countries/Ethiopia.owl"
     xmlns:obo="http://purl.obolibrary.org/obo/"
     xmlns:owl="http://www.w3.org/2002/07/owl#"
     xmlns:rdf="http://www.w3.org/1999/02/22-rdf-syntax-ns#"
     xmlns:xml="http://www.w3.org/XML/1998/namespace"
     xmlns:xsd="http://www.w3.org/2001/XMLSchema#"
     xmlns:rdfs="http://www.w3.org/2000/01/rdf-schema#"
     xmlns:oboInOwl="http://www.geneontology.org/formats/oboInOwl#">
    <owl:Ontology rdf:about="http://purl.obolibrary.org/obo/gaz/subsets/countries/Ethiopia.owl">
        <owl:imports rdf:resource="http://purl.obolibrary.org/obo/gaz/imports/envo_import.owl"/>
        <owl:imports rdf:resource="http://purl.obolibrary.org/obo/gaz/imports/ro_import.owl"/>
    </owl:Ontology>
    


    <!-- 
    ///////////////////////////////////////////////////////////////////////////////////////
    //
    // Annotation properties
    //
    ///////////////////////////////////////////////////////////////////////////////////////
     -->

    


    <!-- http://purl.obolibrary.org/obo/IAO_0000115 -->

    <owl:AnnotationProperty rdf:about="http://purl.obolibrary.org/obo/IAO_0000115"/>
    


    <!-- http://www.geneontology.org/formats/oboInOwl#hasOBONamespace -->

    <owl:AnnotationProperty rdf:about="http://www.geneontology.org/formats/oboInOwl#hasOBONamespace"/>
    


    <!-- http://www.geneontology.org/formats/oboInOwl#id -->

    <owl:AnnotationProperty rdf:about="http://www.geneontology.org/formats/oboInOwl#id"/>
    


    <!-- 
    ///////////////////////////////////////////////////////////////////////////////////////
    //
    // Object Properties
    //
    ///////////////////////////////////////////////////////////////////////////////////////
     -->

    


    <!-- http://purl.obolibrary.org/obo/RO_0001025 -->

    <owl:ObjectProperty rdf:about="http://purl.obolibrary.org/obo/RO_0001025"/>
    


    <!-- 
    ///////////////////////////////////////////////////////////////////////////////////////
    //
    // Classes
    //
    ///////////////////////////////////////////////////////////////////////////////////////
     -->

    


    <!-- http://purl.obolibrary.org/obo/ENVO_00000019 -->

    <owl:Class rdf:about="http://purl.obolibrary.org/obo/ENVO_00000019"/>
    


    <!-- http://purl.obolibrary.org/obo/ENVO_00000032 -->

    <owl:Class rdf:about="http://purl.obolibrary.org/obo/ENVO_00000032"/>
    


    <!-- http://purl.obolibrary.org/obo/ENVO_00000080 -->

    <owl:Class rdf:about="http://purl.obolibrary.org/obo/ENVO_00000080"/>
    


    <!-- http://purl.obolibrary.org/obo/ENVO_00000100 -->

    <owl:Class rdf:about="http://purl.obolibrary.org/obo/ENVO_00000100"/>
    


    <!-- http://purl.obolibrary.org/obo/ENVO_00000106 -->

    <owl:Class rdf:about="http://purl.obolibrary.org/obo/ENVO_00000106"/>
    


    <!-- http://purl.obolibrary.org/obo/ENVO_00000191 -->

    <owl:Class rdf:about="http://purl.obolibrary.org/obo/ENVO_00000191"/>
    


    <!-- http://purl.obolibrary.org/obo/ENVO_00000309 -->

    <owl:Class rdf:about="http://purl.obolibrary.org/obo/ENVO_00000309"/>
    


    <!-- http://purl.obolibrary.org/obo/ENVO_00000354 -->

    <owl:Class rdf:about="http://purl.obolibrary.org/obo/ENVO_00000354"/>
    


    <!-- http://purl.obolibrary.org/obo/ENVO_00000475 -->

    <owl:Class rdf:about="http://purl.obolibrary.org/obo/ENVO_00000475"/>
    


    <!-- http://purl.obolibrary.org/obo/ENVO_00000479 -->

    <owl:Class rdf:about="http://purl.obolibrary.org/obo/ENVO_00000479"/>
    


    <!-- http://purl.obolibrary.org/obo/ENVO_00000856 -->

    <owl:Class rdf:about="http://purl.obolibrary.org/obo/ENVO_00000856"/>
    


    <!-- http://purl.obolibrary.org/obo/GAZ_00000778 -->

    <owl:Class rdf:about="http://purl.obolibrary.org/obo/GAZ_00000778"/>
    


    <!-- http://purl.obolibrary.org/obo/GAZ_00000779 -->

    <owl:Class rdf:about="http://purl.obolibrary.org/obo/GAZ_00000779">
        <rdfs:subClassOf rdf:resource="http://purl.obolibrary.org/obo/GAZ_00000778"/>
    </owl:Class>
    


    <!-- http://purl.obolibrary.org/obo/GAZ_00000780 -->

    <owl:Class rdf:about="http://purl.obolibrary.org/obo/GAZ_00000780">
        <rdfs:subClassOf rdf:resource="http://purl.obolibrary.org/obo/GAZ_00000778"/>
    </owl:Class>
    


    <!-- http://purl.obolibrary.org/obo/GAZ_00000781 -->

    <owl:Class rdf:about="http://purl.obolibrary.org/obo/GAZ_00000781">
        <rdfs:subClassOf rdf:resource="http://purl.obolibrary.org/obo/GAZ_00000778"/>
    </owl:Class>
    


    <!-- http://purl.obolibrary.org/obo/GAZ_00000782 -->

    <owl:Class rdf:about="http://purl.obolibrary.org/obo/GAZ_00000782">
        <rdfs:subClassOf rdf:resource="http://purl.obolibrary.org/obo/GAZ_00000778"/>
    </owl:Class>
    


    <!-- http://purl.obolibrary.org/obo/GAZ_00000783 -->

    <owl:Class rdf:about="http://purl.obolibrary.org/obo/GAZ_00000783">
        <rdfs:subClassOf rdf:resource="http://purl.obolibrary.org/obo/GAZ_00000778"/>
    </owl:Class>
    


    <!-- http://purl.obolibrary.org/obo/GAZ_00000784 -->

    <owl:Class rdf:about="http://purl.obolibrary.org/obo/GAZ_00000784">
        <rdfs:subClassOf rdf:resource="http://purl.obolibrary.org/obo/GAZ_00000778"/>
    </owl:Class>
    


    <!-- http://purl.obolibrary.org/obo/GAZ_00000785 -->

    <owl:Class rdf:about="http://purl.obolibrary.org/obo/GAZ_00000785">
        <rdfs:subClassOf rdf:resource="http://purl.obolibrary.org/obo/GAZ_00000778"/>
    </owl:Class>
    


    <!-- http://purl.obolibrary.org/obo/GAZ_00000786 -->

    <owl:Class rdf:about="http://purl.obolibrary.org/obo/GAZ_00000786">
        <rdfs:subClassOf rdf:resource="http://purl.obolibrary.org/obo/GAZ_00000778"/>
    </owl:Class>
    


    <!-- http://purl.obolibrary.org/obo/GAZ_00000787 -->

    <owl:Class rdf:about="http://purl.obolibrary.org/obo/GAZ_00000787">
        <rdfs:subClassOf rdf:resource="http://purl.obolibrary.org/obo/GAZ_00000778"/>
    </owl:Class>
    


    <!-- http://purl.obolibrary.org/obo/GAZ_00001012 -->

    <owl:Class rdf:about="http://purl.obolibrary.org/obo/GAZ_00001012"/>
    


    <!-- http://purl.obolibrary.org/obo/GAZ_00031091 -->

    <owl:Class rdf:about="http://purl.obolibrary.org/obo/GAZ_00031091">
        <rdfs:subClassOf rdf:resource="http://purl.obolibrary.org/obo/GAZ_00001012"/>
    </owl:Class>
    


    <!-- http://purl.obolibrary.org/obo/GAZ_00031092 -->

    <owl:Class rdf:about="http://purl.obolibrary.org/obo/GAZ_00031092">
        <rdfs:subClassOf rdf:resource="http://purl.obolibrary.org/obo/GAZ_00001012"/>
    </owl:Class>
    


    <!-- http://purl.obolibrary.org/obo/GAZ_00230472 -->

    <owl:Class rdf:about="http://purl.obolibrary.org/obo/GAZ_00230472">
        <obo:IAO_0000115>A river. A tributary of the Qechene River.</obo:IAO_0000115>
        <oboInOwl:hasOBONamespace>GAZ</oboInOwl:hasOBONamespace>
        <oboInOwl:id>GAZ:00230472</oboInOwl:id>
        <rdfs:label>Ketama River</rdfs:label>
    </owl:Class>
    


    <!-- http://purl.obolibrary.org/obo/GAZ_00230473 -->

    <owl:Class rdf:about="http://purl.obolibrary.org/obo/GAZ_00230473">
        <obo:IAO_0000115>A river. A tributary of the Qechene River.</obo:IAO_0000115>
        <oboInOwl:hasOBONamespace>GAZ</oboInOwl:hasOBONamespace>
        <oboInOwl:id>GAZ:00230473</oboInOwl:id>
        <rdfs:label>Woia River</rdfs:label>
    </owl:Class>
    


    <!-- 
    ///////////////////////////////////////////////////////////////////////////////////////
    //
    // Individuals
    //
    ///////////////////////////////////////////////////////////////////////////////////////
     -->

    


    <!-- http://purl.obolibrary.org/obo/GAZ_00000007 -->

    <owl:NamedIndividual rdf:about="http://purl.obolibrary.org/obo/GAZ_00000007">
        <obo:IAO_0000115>A rift valley. A geographical and geological feature, approximately 6,000 km in length, that runs from northern Syria in Southwest Asia to central Mozambique in East Africa.</obo:IAO_0000115>
        <oboInOwl:hasOBONamespace>GAZ</oboInOwl:hasOBONamespace>
        <oboInOwl:id>GAZ:00000007</oboInOwl:id>
        <rdfs:label>Great Rift Valley</rdfs:label>
    </owl:NamedIndividual>
    


    <!-- http://purl.obolibrary.org/obo/GAZ_00000008 -->

    <owl:NamedIndividual rdf:about="http://purl.obolibrary.org/obo/GAZ_00000008">
        <obo:RO_0001025 rdf:resource="http://purl.obolibrary.org/obo/GAZ_00000007"/>
        <obo:IAO_0000115>A soda lake, in the eastern part of the Great Rift Valley. A Ramsar Site.</obo:IAO_0000115>
        <oboInOwl:hasOBONamespace>GAZ</oboInOwl:hasOBONamespace>
        <oboInOwl:id>GAZ:00000008</oboInOwl:id>
        <rdfs:label>Lake Elmenteita</rdfs:label>
    </owl:NamedIndividual>
    


    <!-- http://purl.obolibrary.org/obo/GAZ_00000058 -->

    <owl:NamedIndividual rdf:about="http://purl.obolibrary.org/obo/GAZ_00000058">
        <obo:RO_0001025 rdf:resource="http://purl.obolibrary.org/obo/GAZ_00000007"/>
        <obo:IAO_0000115>A freshwater lake that is the most southerly lake in the Great African Rift Valley system. Its largest tributary is the Ruhuhu and its outlet is the Shire River, a tributary of the Zambezi.</obo:IAO_0000115>
        <oboInOwl:hasOBONamespace>GAZ</oboInOwl:hasOBONamespace>
        <oboInOwl:id>GAZ:00000058</oboInOwl:id>
        <rdfs:label>Lake Malawi</rdfs:label>
    </owl:NamedIndividual>
    


    <!-- http://purl.obolibrary.org/obo/GAZ_00000567 -->

    <owl:NamedIndividual rdf:about="http://purl.obolibrary.org/obo/GAZ_00000567">
        <obo:IAO_0000115>A country situated in the Horn of Africa that has been landlocked since the independence of its northern neighbor Eritrea in 1993. Apart from Eritrea to the north, Ethiopia is bordered by Sudan to the west, Kenya to the south, Djibouti to the northeast, and Somalia to the east. Since 1996 Ethiopia has had a tiered government system consisting of a federal government overseeing ethnically-based regional states, zones, districts (woredas), and neighborhoods (kebele). It is divided into nine ethnically-based administrative states (kililoch, singular kilil) and subdivided into sixty-eight zones and two chartered cities (astedader akababiwoch, singular astedader akababi): Addis Ababa and Dire Dawa. It is further subdivided into 550 woredas and six special woredas.</obo:IAO_0000115>
        <oboInOwl:hasOBONamespace>GAZ</oboInOwl:hasOBONamespace>
        <oboInOwl:id>GAZ:00000567</oboInOwl:id>
        <rdfs:label>Ethiopia</rdfs:label>
    </owl:NamedIndividual>
    


    <!-- http://purl.obolibrary.org/obo/GAZ_00000778 -->

    <owl:NamedIndividual rdf:about="http://purl.obolibrary.org/obo/GAZ_00000778">
        <obo:RO_0001025 rdf:resource="http://purl.obolibrary.org/obo/GAZ_00000567"/>
    </owl:NamedIndividual>
    


    <!-- http://purl.obolibrary.org/obo/GAZ_00000779 -->

    <owl:NamedIndividual rdf:about="http://purl.obolibrary.org/obo/GAZ_00000779"/>
    


    <!-- http://purl.obolibrary.org/obo/GAZ_00000780 -->

    <owl:NamedIndividual rdf:about="http://purl.obolibrary.org/obo/GAZ_00000780"/>
    


    <!-- http://purl.obolibrary.org/obo/GAZ_00000781 -->

    <owl:NamedIndividual rdf:about="http://purl.obolibrary.org/obo/GAZ_00000781"/>
    


    <!-- http://purl.obolibrary.org/obo/GAZ_00000782 -->

    <owl:NamedIndividual rdf:about="http://purl.obolibrary.org/obo/GAZ_00000782"/>
    


    <!-- http://purl.obolibrary.org/obo/GAZ_00000783 -->

    <owl:NamedIndividual rdf:about="http://purl.obolibrary.org/obo/GAZ_00000783"/>
    


    <!-- http://purl.obolibrary.org/obo/GAZ_00000784 -->

    <owl:NamedIndividual rdf:about="http://purl.obolibrary.org/obo/GAZ_00000784"/>
    


    <!-- http://purl.obolibrary.org/obo/GAZ_00000785 -->

    <owl:NamedIndividual rdf:about="http://purl.obolibrary.org/obo/GAZ_00000785"/>
    


    <!-- http://purl.obolibrary.org/obo/GAZ_00000786 -->

    <owl:NamedIndividual rdf:about="http://purl.obolibrary.org/obo/GAZ_00000786"/>
    


    <!-- http://purl.obolibrary.org/obo/GAZ_00000787 -->

    <owl:NamedIndividual rdf:about="http://purl.obolibrary.org/obo/GAZ_00000787"/>
    


    <!-- http://purl.obolibrary.org/obo/GAZ_00000788 -->

    <owl:NamedIndividual rdf:about="http://purl.obolibrary.org/obo/GAZ_00000788">
        <obo:RO_0001025 rdf:resource="http://purl.obolibrary.org/obo/GAZ_00031091"/>
        <oboInOwl:hasOBONamespace>GAZ</oboInOwl:hasOBONamespace>
        <oboInOwl:id>GAZ:00000788</oboInOwl:id>
        <rdfs:label>Addis Ababa Zone 1</rdfs:label>
    </owl:NamedIndividual>
    


    <!-- http://purl.obolibrary.org/obo/GAZ_00000789 -->

    <owl:NamedIndividual rdf:about="http://purl.obolibrary.org/obo/GAZ_00000789">
        <obo:RO_0001025 rdf:resource="http://purl.obolibrary.org/obo/GAZ_00031092"/>
        <obo:IAO_0000115>One of two chartered cities (astedader akabibi) in Ethiopia.</obo:IAO_0000115>
        <oboInOwl:hasOBONamespace>GAZ</oboInOwl:hasOBONamespace>
        <oboInOwl:id>GAZ:00000789</oboInOwl:id>
        <rdfs:label>Dire Dawa</rdfs:label>
    </owl:NamedIndividual>
    


    <!-- http://purl.obolibrary.org/obo/GAZ_00001012 -->

    <owl:NamedIndividual rdf:about="http://purl.obolibrary.org/obo/GAZ_00001012">
        <obo:RO_0001025 rdf:resource="http://purl.obolibrary.org/obo/GAZ_00000567"/>
    </owl:NamedIndividual>
    


    <!-- http://purl.obolibrary.org/obo/GAZ_00002477 -->

    <owl:NamedIndividual rdf:about="http://purl.obolibrary.org/obo/GAZ_00002477">
        <obo:RO_0001025 rdf:resource="http://purl.obolibrary.org/obo/GAZ_00007520"/>
        <obo:IAO_0000115>A saline lake between the West Bank and Israel to the west, and Jordan to the east.</obo:IAO_0000115>
        <oboInOwl:hasOBONamespace>GAZ</oboInOwl:hasOBONamespace>
        <oboInOwl:id>GAZ:00002477</oboInOwl:id>
        <rdfs:label>Dead Sea</rdfs:label>
    </owl:NamedIndividual>
    


    <!-- http://purl.obolibrary.org/obo/GAZ_00003324 -->

    <owl:NamedIndividual rdf:about="http://purl.obolibrary.org/obo/GAZ_00003324">
        <obo:RO_0001025 rdf:resource="http://purl.obolibrary.org/obo/GAZ_00000567"/>
        <oboInOwl:hasOBONamespace>GAZ</oboInOwl:hasOBONamespace>
        <oboInOwl:id>GAZ:00003324</oboInOwl:id>
        <rdfs:label>Ethio tannery</rdfs:label>
    </owl:NamedIndividual>
    


    <!-- http://purl.obolibrary.org/obo/GAZ_00003325 -->

    <owl:NamedIndividual rdf:about="http://purl.obolibrary.org/obo/GAZ_00003325">
        <obo:RO_0001025 rdf:resource="http://purl.obolibrary.org/obo/GAZ_00123414"/>
        <oboInOwl:hasOBONamespace>GAZ</oboInOwl:hasOBONamespace>
        <oboInOwl:id>GAZ:00003325</oboInOwl:id>
        <rdfs:label>Modjo tannery</rdfs:label>
    </owl:NamedIndividual>
    


    <!-- http://purl.obolibrary.org/obo/GAZ_00007520 -->

    <owl:NamedIndividual rdf:about="http://purl.obolibrary.org/obo/GAZ_00007520">
        <obo:RO_0001025 rdf:resource="http://purl.obolibrary.org/obo/GAZ_00044915"/>
        <obo:IAO_0000115>A river in Southwest Asia flowing through the Great Rift Valley into the Dead Sea.</obo:IAO_0000115>
        <oboInOwl:hasOBONamespace>GAZ</oboInOwl:hasOBONamespace>
        <oboInOwl:id>GAZ:00007520</oboInOwl:id>
        <rdfs:label>River Jordan</rdfs:label>
    </owl:NamedIndividual>
    


    <!-- http://purl.obolibrary.org/obo/GAZ_00007523 -->

    <owl:NamedIndividual rdf:about="http://purl.obolibrary.org/obo/GAZ_00007523">
        <obo:RO_0001025 rdf:resource="http://purl.obolibrary.org/obo/GAZ_00000007"/>
        <obo:IAO_0000115>A saline, alkaline lake, approximately 100 km2 in size, that lies in a graben. The lake is an example of a &quot;saline pan&quot;. The lake water, which is a dense sodium carbonate brine, precipitates vast quanitites of the mineral called trona (sodium sesquicarbonate). In places, the salt is up to 40 m thick. The lake is recharged mainly by saline hot springs (temperatures up to about 83degC) that discharge into alkaline &quot;lagoons&quot; around the lake margins, there being little surface runoff in this arid region. Most hot springs lie along the northwestern and southern shorelines of the lake. During the rainy season a thin (&lt;1m) layer of brine covers much of the saline pan, but this evaporates rapidly leaving a vast expanse of white salt that cracks to produce large polygons.</obo:IAO_0000115>
        <oboInOwl:hasOBONamespace>GAZ</oboInOwl:hasOBONamespace>
        <oboInOwl:id>GAZ:00007523</oboInOwl:id>
        <rdfs:label>Lake Magadi</rdfs:label>
    </owl:NamedIndividual>
    


    <!-- http://purl.obolibrary.org/obo/GAZ_00007862 -->

    <owl:NamedIndividual rdf:about="http://purl.obolibrary.org/obo/GAZ_00007862">
        <rdf:type rdf:resource="http://purl.obolibrary.org/obo/ENVO_00000032"/>
        <obo:RO_0001025 rdf:resource="http://purl.obolibrary.org/obo/GAZ_00000007"/>
        <obo:IAO_0000115>A gulf situated northeastward and adjacent to the Red Sea, bounded by the coasts of Sinai Peninsula and Arabian Peninsula. Its southern limit with the Red Sea (in the Strait of T Degrees r Degrees n) is the following: A line joining Cape Al Qa Degrees bah (28 Degrees 01430 Seconds N - 34 Degrees 37 Minutes 15 Seconds E), in Saudi Arabia, southwestward to position 27 Degrees 58 Minutes 10 Seconds N - 34 Degrees 35 Minutes E) on the coast of T Degrees r Degrees n Island; thence from this position southward, through T Degrees r Degrees n Island, to its southwestern extremity (27 Degrees 54 Minutes 50 Seconds N - 34 Degrees 33 Minutes E); and thence from the southwestern extremity of T Degrees r Degrees n Island westward, along the parallel of 27 Degrees 54 Minutes 50 Seconds N, to the coast of Sinai Peninsula, in Egypt.</obo:IAO_0000115>
        <oboInOwl:hasOBONamespace>GAZ</oboInOwl:hasOBONamespace>
        <oboInOwl:id>GAZ:00007862</oboInOwl:id>
        <rdfs:label>Gulf of Aqaba</rdfs:label>
    </owl:NamedIndividual>
    


    <!-- http://purl.obolibrary.org/obo/GAZ_00008411 -->

    <owl:NamedIndividual rdf:about="http://purl.obolibrary.org/obo/GAZ_00008411">
        <obo:RO_0001025 rdf:resource="http://purl.obolibrary.org/obo/GAZ_00000007"/>
        <obo:IAO_0000115>A saline, alkaline lake that lies in a volcanic region in a half-graben basin south of Lake Baringo, Kenya, a little north of the equator. A Ramsar Site.</obo:IAO_0000115>
        <oboInOwl:hasOBONamespace>GAZ</oboInOwl:hasOBONamespace>
        <oboInOwl:id>GAZ:00008411</oboInOwl:id>
        <rdfs:label>Lake Bogoria</rdfs:label>
    </owl:NamedIndividual>
    


    <!-- http://purl.obolibrary.org/obo/GAZ_00008558 -->

    <owl:NamedIndividual rdf:about="http://purl.obolibrary.org/obo/GAZ_00008558">
        <obo:RO_0001025 rdf:resource="http://purl.obolibrary.org/obo/GAZ_00000007"/>
        <obo:IAO_0000115>A meromictic lake that on the border between the Democratic Republic of the Congo and Rwanda, and is in the Albertine (western) Rift, a part of the Great Rift Valley. Lake Kivu empties into the Ruzizi River, which flows southwards into Lake Tanganyika.</obo:IAO_0000115>
        <oboInOwl:hasOBONamespace>GAZ</oboInOwl:hasOBONamespace>
        <oboInOwl:id>GAZ:00008558</oboInOwl:id>
        <rdfs:label>Lake Kivu</rdfs:label>
    </owl:NamedIndividual>
    


    <!-- http://purl.obolibrary.org/obo/GAZ_00008742 -->

    <owl:NamedIndividual rdf:about="http://purl.obolibrary.org/obo/GAZ_00008742">
        <obo:RO_0001025 rdf:resource="http://purl.obolibrary.org/obo/GAZ_00044915"/>
        <obo:IAO_0000115>A valley that lies within the northern part of the Syrian-African Rift Valley at an elevation of about 70 m above sea level. On both sides of the valley are steep slopes -- the Golan Heights to the east and the Upper Galilee mountains to the west, rise to 400 to 900 m above sea level. Basaltic hills of about 200 m above sea level along the southern side of the valley intercept the Jordan River, and are commonly referred to as the basalt &quot;plug&quot; (actually a temporary geologic base level), as they restrict water drainage downstream into the Sea of Galilee (Lake Kinneret). The Hula Valley covers an area of 177 km2 (25 km by 6-8 km.</obo:IAO_0000115>
        <oboInOwl:hasOBONamespace>GAZ</oboInOwl:hasOBONamespace>
        <oboInOwl:id>GAZ:00008742</oboInOwl:id>
        <rdfs:label>Hulah Valley</rdfs:label>
    </owl:NamedIndividual>
    


    <!-- http://purl.obolibrary.org/obo/GAZ_00008743 -->

    <owl:NamedIndividual rdf:about="http://purl.obolibrary.org/obo/GAZ_00008743">
        <obo:RO_0001025 rdf:resource="http://purl.obolibrary.org/obo/GAZ_00193886"/>
        <obo:IAO_0000115>A wetland.</obo:IAO_0000115>
        <oboInOwl:hasOBONamespace>GAZ</oboInOwl:hasOBONamespace>
        <oboInOwl:id>GAZ:00008743</oboInOwl:id>
        <rdfs:label>Hulah Swamp</rdfs:label>
    </owl:NamedIndividual>
    


    <!-- http://purl.obolibrary.org/obo/GAZ_00008747 -->

    <owl:NamedIndividual rdf:about="http://purl.obolibrary.org/obo/GAZ_00008747">
        <rdf:type rdf:resource="http://purl.obolibrary.org/obo/ENVO_00000856"/>
        <obo:RO_0001025 rdf:resource="http://purl.obolibrary.org/obo/GAZ_00052535"/>
        <obo:IAO_0000115>A populated place. A town in northern Ethiopia.</obo:IAO_0000115>
        <oboInOwl:hasOBONamespace>GAZ</oboInOwl:hasOBONamespace>
        <oboInOwl:id>GAZ:00008747</oboInOwl:id>
        <rdfs:label>Lalibela</rdfs:label>
    </owl:NamedIndividual>
    


    <!-- http://purl.obolibrary.org/obo/GAZ_00009142 -->

    <owl:NamedIndividual rdf:about="http://purl.obolibrary.org/obo/GAZ_00009142">
        <obo:RO_0001025 rdf:resource="http://purl.obolibrary.org/obo/GAZ_00008558"/>
        <obo:IAO_0000115>An island in Lake Kivu, belonging to the Democratic Republic of the Congo. At 40 km in length and with an area of 285 km2.</obo:IAO_0000115>
        <oboInOwl:hasOBONamespace>GAZ</oboInOwl:hasOBONamespace>
        <oboInOwl:id>GAZ:00009142</oboInOwl:id>
        <rdfs:label>Idjwi Island</rdfs:label>
    </owl:NamedIndividual>
    


    <!-- http://purl.obolibrary.org/obo/GAZ_00010533 -->

    <owl:NamedIndividual rdf:about="http://purl.obolibrary.org/obo/GAZ_00010533">
        <obo:RO_0001025 rdf:resource="http://purl.obolibrary.org/obo/GAZ_00044915"/>
        <obo:IAO_0000115>A large fertile plain and inland valley in the south of the Lower Galilee region of Israel. It is bordered to the south by the Samaria highlands and Mount Gilboa, to the north by the Lower Galilee, to the west by the Mount Carmel range, and to the east by the Jordan Valley.</obo:IAO_0000115>
        <oboInOwl:hasOBONamespace>GAZ</oboInOwl:hasOBONamespace>
        <oboInOwl:id>GAZ:00010533</oboInOwl:id>
        <rdfs:label>Jezreel Valley</rdfs:label>
    </owl:NamedIndividual>
    


    <!-- http://purl.obolibrary.org/obo/GAZ_00011722 -->

    <owl:NamedIndividual rdf:about="http://purl.obolibrary.org/obo/GAZ_00011722">
        <obo:RO_0001025 rdf:resource="http://purl.obolibrary.org/obo/GAZ_00000007"/>
        <obo:IAO_0000115>A freshwater lake is situated within the Western Rift of the Great Rift Valley. The major inflows are the Ruzizi River, entering the north of the lake from Lake Kivu, and the Malagarasi River, which is Tanzania&apos;s second largest river, entering in the east side of Lake Tanganyika. The Malagarasi pre-dates Lake Tanganyika and was formerly continuous with the Congo river.</obo:IAO_0000115>
        <oboInOwl:hasOBONamespace>GAZ</oboInOwl:hasOBONamespace>
        <oboInOwl:id>GAZ:00011722</oboInOwl:id>
        <rdfs:label>Lake Tanganyika</rdfs:label>
    </owl:NamedIndividual>
    


    <!-- http://purl.obolibrary.org/obo/GAZ_00015452 -->

    <owl:NamedIndividual rdf:about="http://purl.obolibrary.org/obo/GAZ_00015452">
        <obo:RO_0001025 rdf:resource="http://purl.obolibrary.org/obo/GAZ_00000007"/>
        <obo:IAO_0000115>A very large monictic freshwater lake bordering Kenya, Tanzania and Uganda.</obo:IAO_0000115>
        <oboInOwl:hasOBONamespace>GAZ</oboInOwl:hasOBONamespace>
        <oboInOwl:id>GAZ:00015452</oboInOwl:id>
        <rdfs:label>Lake Victoria</rdfs:label>
    </owl:NamedIndividual>
    


    <!-- http://purl.obolibrary.org/obo/GAZ_00015453 -->

    <owl:NamedIndividual rdf:about="http://purl.obolibrary.org/obo/GAZ_00015453">
        <obo:RO_0001025 rdf:resource="http://purl.obolibrary.org/obo/GAZ_00124567"/>
        <obo:IAO_0000115>A chain of more than fifty smaller islands, a few km off the northern shore of Lake Victoria, Uganda in the Napoleon Gulf.</obo:IAO_0000115>
        <oboInOwl:hasOBONamespace>GAZ</oboInOwl:hasOBONamespace>
        <oboInOwl:id>GAZ:00015453</oboInOwl:id>
        <rdfs:label>Buvuma Islands</rdfs:label>
    </owl:NamedIndividual>
    


    <!-- http://purl.obolibrary.org/obo/GAZ_00029996 -->

    <owl:NamedIndividual rdf:about="http://purl.obolibrary.org/obo/GAZ_00029996">
        <obo:RO_0001025 rdf:resource="http://purl.obolibrary.org/obo/GAZ_00000058"/>
        <obo:IAO_0000115>The smaller of two inhabited islands in Lake Malawi. It lies just a few km from Mozambique, and is entirely surrounded by Mozambican territorial waters, but belongs to Malawi.It is, therefore, an exclave of Malawi.</obo:IAO_0000115>
        <oboInOwl:hasOBONamespace>GAZ</oboInOwl:hasOBONamespace>
        <oboInOwl:id>GAZ:00029996</oboInOwl:id>
        <rdfs:label>Chisumulu Island</rdfs:label>
    </owl:NamedIndividual>
    


    <!-- http://purl.obolibrary.org/obo/GAZ_00029997 -->

    <owl:NamedIndividual rdf:about="http://purl.obolibrary.org/obo/GAZ_00029997">
        <obo:RO_0001025 rdf:resource="http://purl.obolibrary.org/obo/GAZ_00000058"/>
        <obo:IAO_0000115>The larger of two inhabited islands in Lake Malawi. It lies just a few km from Mozambique, and is surrounded by Mozambican territorial waters, but belongs to Malawi. An exclave of Malawi.</obo:IAO_0000115>
        <oboInOwl:hasOBONamespace>GAZ</oboInOwl:hasOBONamespace>
        <oboInOwl:id>GAZ:00029997</oboInOwl:id>
        <rdfs:label>Likoma Island</rdfs:label>
    </owl:NamedIndividual>
    


    <!-- http://purl.obolibrary.org/obo/GAZ_00031086 -->

    <owl:NamedIndividual rdf:about="http://purl.obolibrary.org/obo/GAZ_00031086">
        <obo:RO_0001025 rdf:resource="http://purl.obolibrary.org/obo/GAZ_00000779"/>
        <obo:IAO_0000115>One of five Zones of the Afar Region of Ethiopia. This zone is bordered on the south by Administrative Zone 4, on the southwest by Administrative Zone 1, on the west by the Amhara Region, and on the northeast by Eritrea.</obo:IAO_0000115>
        <oboInOwl:hasOBONamespace>GAZ</oboInOwl:hasOBONamespace>
        <oboInOwl:id>GAZ:00031086</oboInOwl:id>
        <rdfs:label>Afar Zone 2</rdfs:label>
    </owl:NamedIndividual>
    


    <!-- http://purl.obolibrary.org/obo/GAZ_00031087 -->

    <owl:NamedIndividual rdf:about="http://purl.obolibrary.org/obo/GAZ_00031087">
        <obo:RO_0001025 rdf:resource="http://purl.obolibrary.org/obo/GAZ_00000779"/>
        <obo:IAO_0000115>One of five Zones of the Afar Region of Ethiopia; none of the zones of Afar have names. This zone is bordered on the south by Administrative Zone 3, on the southwest by Administrative Zone 5, on the west by the Amhara Region, on the northwest by Administrative Zones 4 and 2, on the north by Eritrea, and on the east by Djibouti.</obo:IAO_0000115>
        <oboInOwl:hasOBONamespace>GAZ</oboInOwl:hasOBONamespace>
        <oboInOwl:id>GAZ:00031087</oboInOwl:id>
        <rdfs:label>Afar Zone 1</rdfs:label>
    </owl:NamedIndividual>
    


    <!-- http://purl.obolibrary.org/obo/GAZ_00031088 -->

    <owl:NamedIndividual rdf:about="http://purl.obolibrary.org/obo/GAZ_00031088">
        <obo:RO_0001025 rdf:resource="http://purl.obolibrary.org/obo/GAZ_00000779"/>
        <obo:IAO_0000115>One of five Zones of the Afar Region of Ethiopia; none of the zones of Afar have names. This zone is bordered on the south and east by Administrative Zone 1, on the west by the Amhara Region, and on the north by Administrative Zone 2. The largest town in Zone 4 is Dibina.</obo:IAO_0000115>
        <oboInOwl:hasOBONamespace>GAZ</oboInOwl:hasOBONamespace>
        <oboInOwl:id>GAZ:00031088</oboInOwl:id>
        <rdfs:label>Afar Zone 4</rdfs:label>
    </owl:NamedIndividual>
    


    <!-- http://purl.obolibrary.org/obo/GAZ_00031089 -->

    <owl:NamedIndividual rdf:about="http://purl.obolibrary.org/obo/GAZ_00031089">
        <obo:RO_0001025 rdf:resource="http://purl.obolibrary.org/obo/GAZ_00000779"/>
        <obo:IAO_0000115>One of five Zones of the Afar Region of Ethiopia; none of the zones of Afar have names. This zone is bordered on the south by the Oromia Region, on the southwest by the Amhara Region, on the west by the Argobba special woreda and the Awash River which separates it from Administrative Zone 5, on the north by Administrative Zone 1, and on the east by the Somali Region.</obo:IAO_0000115>
        <oboInOwl:hasOBONamespace>GAZ</oboInOwl:hasOBONamespace>
        <oboInOwl:id>GAZ:00031089</oboInOwl:id>
        <rdfs:label>Afar Zone 3</rdfs:label>
    </owl:NamedIndividual>
    


    <!-- http://purl.obolibrary.org/obo/GAZ_00031090 -->

    <owl:NamedIndividual rdf:about="http://purl.obolibrary.org/obo/GAZ_00031090">
        <obo:RO_0001025 rdf:resource="http://purl.obolibrary.org/obo/GAZ_00000779"/>
        <obo:IAO_0000115>One of five Zones of the Afar Region of Ethiopia. It is stretching along the eastern base of the Ethiopian highlands. It is bordered on the south and east by Administrative Zone 3, on the west by the Amhara Region, and on the north by Administrative Zone 1.</obo:IAO_0000115>
        <oboInOwl:hasOBONamespace>GAZ</oboInOwl:hasOBONamespace>
        <oboInOwl:id>GAZ:00031090</oboInOwl:id>
        <rdfs:label>Afar Zone 5</rdfs:label>
    </owl:NamedIndividual>
    


    <!-- http://purl.obolibrary.org/obo/GAZ_00031091 -->

    <owl:NamedIndividual rdf:about="http://purl.obolibrary.org/obo/GAZ_00031091"/>
    


    <!-- http://purl.obolibrary.org/obo/GAZ_00031092 -->

    <owl:NamedIndividual rdf:about="http://purl.obolibrary.org/obo/GAZ_00031092"/>
    


    <!-- http://purl.obolibrary.org/obo/GAZ_00031093 -->

    <owl:NamedIndividual rdf:about="http://purl.obolibrary.org/obo/GAZ_00031093">
        <obo:RO_0001025 rdf:resource="http://purl.obolibrary.org/obo/GAZ_00000780"/>
        <obo:IAO_0000115>One of 10 Zones in the Ethiopian Amhara Region. Semen Shewa is bordered on the south and the west by the Oromia Region, on the north by Debub Wollo, on the northeast by the Oromia Zone, and on the east by the Afar Region. Towns and cities in Semen Shewa include Ankober, Debre Berhan, and Shewa Robit.</obo:IAO_0000115>
        <oboInOwl:hasOBONamespace>GAZ</oboInOwl:hasOBONamespace>
        <oboInOwl:id>GAZ:00031093</oboInOwl:id>
        <rdfs:label>North Shewa Zone</rdfs:label>
    </owl:NamedIndividual>
    


    <!-- http://purl.obolibrary.org/obo/GAZ_00031094 -->

    <owl:NamedIndividual rdf:about="http://purl.obolibrary.org/obo/GAZ_00031094">
        <obo:RO_0001025 rdf:resource="http://purl.obolibrary.org/obo/GAZ_00000780"/>
        <obo:IAO_0000115>One of 10 Zones in the Ethiopian Amhara Region. Debub Wollo is bordered on the south by Semien Shewa and the Oromia Region, on the west by Mirab Gojjam, on the northwest by Debub Gondar, on the north by Semien Wollo and on the east by the Oromia Zone.</obo:IAO_0000115>
        <oboInOwl:hasOBONamespace>GAZ</oboInOwl:hasOBONamespace>
        <oboInOwl:id>GAZ:00031094</oboInOwl:id>
        <rdfs:label>South Wollo Zone</rdfs:label>
    </owl:NamedIndividual>
    


    <!-- http://purl.obolibrary.org/obo/GAZ_00031095 -->

    <owl:NamedIndividual rdf:about="http://purl.obolibrary.org/obo/GAZ_00031095">
        <obo:RO_0001025 rdf:resource="http://purl.obolibrary.org/obo/GAZ_00000780"/>
        <obo:IAO_0000115>One of 10 Zones in the Amhara Region of Ethiopia. Oromia is bordered on the southwest by Semien Shewa, on the northwest by Debub Wollo, and on the east by the Afar Region. Towns in Oromia include Bati and Kemise, which is the administrative center of the zone.</obo:IAO_0000115>
        <oboInOwl:hasOBONamespace>GAZ</oboInOwl:hasOBONamespace>
        <oboInOwl:id>GAZ:00031095</oboInOwl:id>
        <rdfs:label>Oromiya Zone</rdfs:label>
    </owl:NamedIndividual>
    


    <!-- http://purl.obolibrary.org/obo/GAZ_00031096 -->

    <owl:NamedIndividual rdf:about="http://purl.obolibrary.org/obo/GAZ_00031096">
        <obo:RO_0001025 rdf:resource="http://purl.obolibrary.org/obo/GAZ_00000780"/>
        <obo:IAO_0000115>A special zone. Bahir Dar is situated on the southern shore of Lake Tana.</obo:IAO_0000115>
        <oboInOwl:hasOBONamespace>GAZ</oboInOwl:hasOBONamespace>
        <oboInOwl:id>GAZ:00031096</oboInOwl:id>
        <rdfs:label>Bahir Dar Special Zone</rdfs:label>
    </owl:NamedIndividual>
    


    <!-- http://purl.obolibrary.org/obo/GAZ_00031097 -->

    <owl:NamedIndividual rdf:about="http://purl.obolibrary.org/obo/GAZ_00031097">
        <obo:RO_0001025 rdf:resource="http://purl.obolibrary.org/obo/GAZ_00000780"/>
        <obo:IAO_0000115>A Zone in the Amhara Region of Ethiopia. Wag Hemra is bordered on the south by Semien Wollo, on the southwest by Debub (South) Gondar, on the west by Semen (North) Gondar, on the north and east by the Tigray Region. Towns in Wag Hemra include Soqota.</obo:IAO_0000115>
        <oboInOwl:hasOBONamespace>GAZ</oboInOwl:hasOBONamespace>
        <oboInOwl:id>GAZ:00031097</oboInOwl:id>
        <rdfs:label>Wag Hemra Zone</rdfs:label>
    </owl:NamedIndividual>
    


    <!-- http://purl.obolibrary.org/obo/GAZ_00031098 -->

    <owl:NamedIndividual rdf:about="http://purl.obolibrary.org/obo/GAZ_00031098">
        <obo:RO_0001025 rdf:resource="http://purl.obolibrary.org/obo/GAZ_00000780"/>
        <obo:IAO_0000115>One of 10 Zones in the Amhara Region of Ethiopia. Agew Awi is bordered on the south by the Oromia Region, on the west by Benishangul-Gumuz Region, on the north-west by Semien Gondar Zone and on the north and east by Misraq Gojjam. The administrative center of Agew Awi is Injibara.</obo:IAO_0000115>
        <oboInOwl:hasOBONamespace>GAZ</oboInOwl:hasOBONamespace>
        <oboInOwl:id>GAZ:00031098</oboInOwl:id>
        <rdfs:label>Agew Awi Zone</rdfs:label>
    </owl:NamedIndividual>
    


    <!-- http://purl.obolibrary.org/obo/GAZ_00031099 -->

    <owl:NamedIndividual rdf:about="http://purl.obolibrary.org/obo/GAZ_00031099">
        <obo:RO_0001025 rdf:resource="http://purl.obolibrary.org/obo/GAZ_00000780"/>
        <obo:IAO_0000115>A Zone in the Ethiopian Amhara Region. Semien Gondar is bordered on the south by Lake Tana, Mirab (West) Gojjam and the Benishangul-Gumuz Region, on the west by Sudan, on the north by the Tigray Region, on the east by Wag Hemra and on the southeast by Debub Gondar. Towns and cities in Semien Gondar include Debarq, Emfranz, Gondar, Gorgora and Metemma.</obo:IAO_0000115>
        <oboInOwl:hasOBONamespace>GAZ</oboInOwl:hasOBONamespace>
        <oboInOwl:id>GAZ:00031099</oboInOwl:id>
        <rdfs:label>North Gonder Zone</rdfs:label>
    </owl:NamedIndividual>
    


    <!-- http://purl.obolibrary.org/obo/GAZ_00031100 -->

    <owl:NamedIndividual rdf:about="http://purl.obolibrary.org/obo/GAZ_00031100">
        <obo:RO_0001025 rdf:resource="http://purl.obolibrary.org/obo/GAZ_00000780"/>
        <obo:IAO_0000115>A Zone in the Amhara Region of Ethiopia. Mirab Gojjam is named after the former province of Gojjam. Mirab Gojjam is bordered on the south by the Abay River which separates it from the Oromia Region, on the west by Agew Awi, on the northwest by Semien Gondar, on the north by Lake Tana, on the northeast by Bahir Dar and the Abay River which separates it from the Debub Gondar, and on the east by Misraq Gojjam. Its highest point is Mount Amedamit. Towns and cities in Mirab Gojjam include Adet, Finote Selam, and Bure.</obo:IAO_0000115>
        <oboInOwl:hasOBONamespace>GAZ</oboInOwl:hasOBONamespace>
        <oboInOwl:id>GAZ:00031100</oboInOwl:id>
        <rdfs:label>West Gojam Zone</rdfs:label>
    </owl:NamedIndividual>
    


    <!-- http://purl.obolibrary.org/obo/GAZ_00031101 -->

    <owl:NamedIndividual rdf:about="http://purl.obolibrary.org/obo/GAZ_00031101">
        <obo:RO_0001025 rdf:resource="http://purl.obolibrary.org/obo/GAZ_00000780"/>
        <obo:IAO_0000115>A Zone in the Ethiopian Amhara Region. Semien Wollo acquired its name from the former province of Wollo. Semien Wello is bordered on the south by Debub Wollo, on the west by Debub Gondar, on the north by Wag Hemra, and on the northeast and east by the Afar Region. Towns and cities in Semen Wello include Lalibela and Weldiya.</obo:IAO_0000115>
        <oboInOwl:hasOBONamespace>GAZ</oboInOwl:hasOBONamespace>
        <oboInOwl:id>GAZ:00031101</oboInOwl:id>
        <rdfs:label>North Wollo Zone</rdfs:label>
    </owl:NamedIndividual>
    


    <!-- http://purl.obolibrary.org/obo/GAZ_00031102 -->

    <owl:NamedIndividual rdf:about="http://purl.obolibrary.org/obo/GAZ_00031102">
        <obo:RO_0001025 rdf:resource="http://purl.obolibrary.org/obo/GAZ_00000780"/>
        <obo:IAO_0000115>A Zone in the Ethiopian Amhara Region. Debub Gondar is bordered on the south by Misraq Gojjam, on the southwest by Misrab Gojjam and Bahir Dar, on the west by Lake Tana, on the north by Semien Gondar, on the northeast by Wag Hemra, on the east by Semien Wollo, and on the southeast by Debub Wollo; the Abbay River separates Debub Gondar from the two Gojjam Zones.</obo:IAO_0000115>
        <oboInOwl:hasOBONamespace>GAZ</oboInOwl:hasOBONamespace>
        <oboInOwl:id>GAZ:00031102</oboInOwl:id>
        <rdfs:label>South Gonder Zone</rdfs:label>
    </owl:NamedIndividual>
    


    <!-- http://purl.obolibrary.org/obo/GAZ_00031103 -->

    <owl:NamedIndividual rdf:about="http://purl.obolibrary.org/obo/GAZ_00031103">
        <obo:RO_0001025 rdf:resource="http://purl.obolibrary.org/obo/GAZ_00000780"/>
        <obo:IAO_0000115>A Zone in the Amhara Region of Ethiopia. Misraq Gojjam is named after the former province of Gojjam. Misraq Gojjam is bordered on the south by the Oromia Region, on the west by Mirab Gojjam, on the north by Debub Gondar, and on the east by Debub Wollo; the bend of the Abay River defines the Zone&apos;s northern, eastern and southern boundaries. Its highest point is Mount Choqa (also known as Mount Birhan). Towns and cities in Misraq Gojjam include Bichena, Debre Marqos, Debre Werq, and Mota.</obo:IAO_0000115>
        <oboInOwl:hasOBONamespace>GAZ</oboInOwl:hasOBONamespace>
        <oboInOwl:id>GAZ:00031103</oboInOwl:id>
        <rdfs:label>East Gojam Zone</rdfs:label>
    </owl:NamedIndividual>
    


    <!-- http://purl.obolibrary.org/obo/GAZ_00031104 -->

    <owl:NamedIndividual rdf:about="http://purl.obolibrary.org/obo/GAZ_00031104">
        <obo:RO_0001025 rdf:resource="http://purl.obolibrary.org/obo/GAZ_00000781"/>
        <obo:IAO_0000115>One of the three Zones in Benishangul-Gumuz Region of Ethiopia. Asosa is bordered on the south by the Mao-Komo special woreda, on the west by Sudan, on the northeast by the Abay River which separates it from Metekel, and on the east by the Dabus River which separates it from Kamashi. The largest town in this zone is Asosa. Its highest point is Mount Bambasi, located in the woreda of the same name.</obo:IAO_0000115>
        <oboInOwl:hasOBONamespace>GAZ</oboInOwl:hasOBONamespace>
        <oboInOwl:id>GAZ:00031104</oboInOwl:id>
        <rdfs:label>Asosa Zone</rdfs:label>
    </owl:NamedIndividual>
    


    <!-- http://purl.obolibrary.org/obo/GAZ_00031105 -->

    <owl:NamedIndividual rdf:about="http://purl.obolibrary.org/obo/GAZ_00031105">
        <obo:RO_0001025 rdf:resource="http://purl.obolibrary.org/obo/GAZ_00000781"/>
        <obo:IAO_0000115>One of the three Zones in the Benishangul-Gumuz Region of Ethiopia. Metekel is bordered on the south by Kamashi, on the southwest by Asosa, on the west by Sudan, and on the north and east by the Amhara Region. The Abay River defines the zone&apos;s boundaries with Kamashi and Asosa, while the Dinder River defines part of its boundary with the Amhara Region.</obo:IAO_0000115>
        <oboInOwl:hasOBONamespace>GAZ</oboInOwl:hasOBONamespace>
        <oboInOwl:id>GAZ:00031105</oboInOwl:id>
        <rdfs:label>Metekel Zone</rdfs:label>
    </owl:NamedIndividual>
    


    <!-- http://purl.obolibrary.org/obo/GAZ_00031106 -->

    <owl:NamedIndividual rdf:about="http://purl.obolibrary.org/obo/GAZ_00031106">
        <obo:RO_0001025 rdf:resource="http://purl.obolibrary.org/obo/GAZ_00000781"/>
        <obo:IAO_0000115>One of the 22 woredas in the Benishangul-Gumuz Region of Ethiopia. Because Mao-Komo is not part of any Zone in Benishangul-Gumuz, it is considered a Special woreda. The southernmost woreda in the Region, Mao-Komo is bordered on the west by Sudan, on the north by the Asosa Zone, and on the east and south by the Oromia Region.</obo:IAO_0000115>
        <oboInOwl:hasOBONamespace>GAZ</oboInOwl:hasOBONamespace>
        <oboInOwl:id>GAZ:00031106</oboInOwl:id>
        <rdfs:label>Mao-Komo special Woreda</rdfs:label>
    </owl:NamedIndividual>
    


    <!-- http://purl.obolibrary.org/obo/GAZ_00031107 -->

    <owl:NamedIndividual rdf:about="http://purl.obolibrary.org/obo/GAZ_00031107">
        <obo:RO_0001025 rdf:resource="http://purl.obolibrary.org/obo/GAZ_00000781"/>
        <obo:IAO_0000115>One of the three Zones in the Benishangul-Gumuz Region of Ethiopia. Kamashi coverss part of the southern bank of the Abay and the valley of the Didessa Rivers; it is bordered on the south and east by the Oromia Region, on the west by the Dabus River which separates it from Asosa and on the north by Metekel and the Amhara Region, which lie on the further bank of the Abay.</obo:IAO_0000115>
        <oboInOwl:hasOBONamespace>GAZ</oboInOwl:hasOBONamespace>
        <oboInOwl:id>GAZ:00031107</oboInOwl:id>
        <rdfs:label>Kamashi Zone</rdfs:label>
    </owl:NamedIndividual>
    


    <!-- http://purl.obolibrary.org/obo/GAZ_00031108 -->

    <owl:NamedIndividual rdf:about="http://purl.obolibrary.org/obo/GAZ_00031108">
        <obo:RO_0001025 rdf:resource="http://purl.obolibrary.org/obo/GAZ_00000782"/>
        <obo:IAO_0000115>One of the zones of the Ethiopian Region of Gambela; none of the zones of Gambela have names. This zone is bordered on the south by Administrative Zone 2, on the west by Administrative Zone 3 and on the north and east by the Oromia Region. Towns and cities in this zone include Itang and Gambela.</obo:IAO_0000115>
        <oboInOwl:hasOBONamespace>GAZ</oboInOwl:hasOBONamespace>
        <oboInOwl:id>GAZ:00031108</oboInOwl:id>
        <rdfs:label>Gambella Zone 1</rdfs:label>
    </owl:NamedIndividual>
    


    <!-- http://purl.obolibrary.org/obo/GAZ_00031109 -->

    <owl:NamedIndividual rdf:about="http://purl.obolibrary.org/obo/GAZ_00031109">
        <obo:RO_0001025 rdf:resource="http://purl.obolibrary.org/obo/GAZ_00000782"/>
        <obo:IAO_0000115>One of the zones of the Ethiopian Region of Gambela; none of the zones of Gambela have names. This zone is bordered by Sudan on the south, west and north, by Administrative Zone 1 on the east and Administrative Zone 2 on the southeast. Towns and cities in this zone include Tergol and Telut.</obo:IAO_0000115>
        <oboInOwl:hasOBONamespace>GAZ</oboInOwl:hasOBONamespace>
        <oboInOwl:id>GAZ:00031109</oboInOwl:id>
        <rdfs:label>Gambella Zone 3</rdfs:label>
    </owl:NamedIndividual>
    


    <!-- http://purl.obolibrary.org/obo/GAZ_00031110 -->

    <owl:NamedIndividual rdf:about="http://purl.obolibrary.org/obo/GAZ_00031110">
        <obo:RO_0001025 rdf:resource="http://purl.obolibrary.org/obo/GAZ_00000782"/>
        <obo:IAO_0000115>One of the zones of the Ethiopian Region of Gambela; none of the zones of Gambela have names.</obo:IAO_0000115>
        <oboInOwl:hasOBONamespace>GAZ</oboInOwl:hasOBONamespace>
        <oboInOwl:id>GAZ:00031110</oboInOwl:id>
        <rdfs:label>Gambella Zone 4</rdfs:label>
    </owl:NamedIndividual>
    


    <!-- http://purl.obolibrary.org/obo/GAZ_00031111 -->

    <owl:NamedIndividual rdf:about="http://purl.obolibrary.org/obo/GAZ_00031111">
        <obo:RO_0001025 rdf:resource="http://purl.obolibrary.org/obo/GAZ_00000782"/>
        <obo:IAO_0000115>One of the zones of the Ethiopian Region of Gambela; none of the zones of Gambela have names. This zone is bordered by Sudan and the Southern Nations, Nationalities, and Peoples Region on the south, Administrative Zone 3 on the west, Administrative Zone 1 on the north, and the Godere special woreda on the east. Towns in this zone include Abobo and Fugnido.</obo:IAO_0000115>
        <oboInOwl:hasOBONamespace>GAZ</oboInOwl:hasOBONamespace>
        <oboInOwl:id>GAZ:00031111</oboInOwl:id>
        <rdfs:label>Gambella Zone 2</rdfs:label>
    </owl:NamedIndividual>
    


    <!-- http://purl.obolibrary.org/obo/GAZ_00031112 -->

    <owl:NamedIndividual rdf:about="http://purl.obolibrary.org/obo/GAZ_00031112">
        <obo:RO_0001025 rdf:resource="http://purl.obolibrary.org/obo/GAZ_00000783"/>
        <oboInOwl:hasOBONamespace>GAZ</oboInOwl:hasOBONamespace>
        <oboInOwl:id>GAZ:00031112</oboInOwl:id>
        <rdfs:label>Harari Zone</rdfs:label>
    </owl:NamedIndividual>
    


    <!-- http://purl.obolibrary.org/obo/GAZ_00031113 -->

    <owl:NamedIndividual rdf:about="http://purl.obolibrary.org/obo/GAZ_00031113">
        <obo:RO_0001025 rdf:resource="http://purl.obolibrary.org/obo/GAZ_00000784"/>
        <obo:IAO_0000115>One of the 12 zones of the Oromia Region of Ethiopia. Borena is bordered on the south by Kenya, on the west by the Southern Nations, Nationalities, and Peoples Region, on the north by the Ganale Dorya River which separates it from Bale and on the east by the Somali Region. The highest point in this zone is Mount Dara Tiniro. Cities and major towns in this Zone include Moyale, Negele Boran, and Yabelo.</obo:IAO_0000115>
        <oboInOwl:hasOBONamespace>GAZ</oboInOwl:hasOBONamespace>
        <oboInOwl:id>GAZ:00031113</oboInOwl:id>
        <rdfs:label>Borena Zone</rdfs:label>
    </owl:NamedIndividual>
    


    <!-- http://purl.obolibrary.org/obo/GAZ_00031114 -->

    <owl:NamedIndividual rdf:about="http://purl.obolibrary.org/obo/GAZ_00031114">
        <obo:RO_0001025 rdf:resource="http://purl.obolibrary.org/obo/GAZ_00000784"/>
        <obo:IAO_0000115>One of the 12 Zones in the Oromia Region of Ethiopia. Bale is named for the former kingdom of Bale, which is located in approximately the same area. Bale is bordered on the south by the Ganale Dorya River which separates it from Borena, on the southwest by the Southern Nations, Nationalities and Peoples Region, on the northwest by Arsi, on the northeast by the Shebelle River which separates it from Mirab Hararghe and Misraq Hararghe, and on the east by the Somali Region. The highest point in the Bale Zone, and also the highest point in Oromia, is Mount Batu (4,307 m), one of the Urgoma Mountains. Other notable peaks of the Urgoma include Mount Tullu Demtu, Mount Darkeena and Mount Gaysay. Towns and cities in Bale include Dodola, Ginir, Goba and Robe.</obo:IAO_0000115>
        <oboInOwl:hasOBONamespace>GAZ</oboInOwl:hasOBONamespace>
        <oboInOwl:id>GAZ:00031114</oboInOwl:id>
        <rdfs:label>Bale Zone</rdfs:label>
    </owl:NamedIndividual>
    


    <!-- http://purl.obolibrary.org/obo/GAZ_00031115 -->

    <owl:NamedIndividual rdf:about="http://purl.obolibrary.org/obo/GAZ_00031115">
        <obo:RO_0001025 rdf:resource="http://purl.obolibrary.org/obo/GAZ_00000785"/>
        <obo:IAO_0000115>One of nine Zones of the Somali Region of Ethiopia. Fiq is bordered on the south by Gode, on the west and north by the Oromia Region, and on the east by Degehabur. The western border is defined by the course of the Erer River.</obo:IAO_0000115>
        <oboInOwl:hasOBONamespace>GAZ</oboInOwl:hasOBONamespace>
        <oboInOwl:id>GAZ:00031115</oboInOwl:id>
        <rdfs:label>Fik Zone</rdfs:label>
    </owl:NamedIndividual>
    


    <!-- http://purl.obolibrary.org/obo/GAZ_00031116 -->

    <owl:NamedIndividual rdf:about="http://purl.obolibrary.org/obo/GAZ_00031116">
        <obo:RO_0001025 rdf:resource="http://purl.obolibrary.org/obo/GAZ_00000784"/>
        <obo:IAO_0000115>One of the 12 Zones of the Ethiopian Region of Oromia. Misraq Hararge takes its name from the former province of Hararghe. Misrak Harerge is bordered on the southwest by the Shebelle River which separates it from Bale, on the west by Mirab Hararghe, on the north by Dire Dawa and on the north and east by the Somali Region. The Harari Region is an enclave inside this zone.</obo:IAO_0000115>
        <oboInOwl:hasOBONamespace>GAZ</oboInOwl:hasOBONamespace>
        <oboInOwl:id>GAZ:00031116</oboInOwl:id>
        <rdfs:label>East Harerge Zone</rdfs:label>
    </owl:NamedIndividual>
    


    <!-- http://purl.obolibrary.org/obo/GAZ_00031117 -->

    <owl:NamedIndividual rdf:about="http://purl.obolibrary.org/obo/GAZ_00031117">
        <obo:RO_0001025 rdf:resource="http://purl.obolibrary.org/obo/GAZ_00000784"/>
        <obo:IAO_0000115>One of the 12 zones of the Oromia Region in Ethiopia. Arsi is bordered on the south by Bale, on the southwest by the Southern Nations, Nationalities, and People&apos;s Region, on the northwest by Misraq (East) Shewa, on the north by the Afar Region and on the east by Mirab (West) Hararghe. The highest point in Arsi is Mount Chilalo; other notable mountains in this zone include Mount Kaka and Mount Gugu. The administrative center of this zone is in Asella; other towns in this zone include Abomsa and Asasa.</obo:IAO_0000115>
        <oboInOwl:hasOBONamespace>GAZ</oboInOwl:hasOBONamespace>
        <oboInOwl:id>GAZ:00031117</oboInOwl:id>
        <rdfs:label>Arsi Zone</rdfs:label>
    </owl:NamedIndividual>
    


    <!-- http://purl.obolibrary.org/obo/GAZ_00031118 -->

    <owl:NamedIndividual rdf:about="http://purl.obolibrary.org/obo/GAZ_00031118">
        <obo:RO_0001025 rdf:resource="http://purl.obolibrary.org/obo/GAZ_00000784"/>
        <obo:IAO_0000115>A Zone in the Ethiopian Region of Oromia. Jimma is bordered on the south by the Southern Nations, Nationalities and Peoples Region, the northwest by Illubabor, on the north by Mirab Welega, and on the northeast by Misraq Shewa; part of the boundary with Misraq Shewa is defined by the Gibe River. The highest point in this zone is Mount Maigudo (2,386 m). Towns and cities in Jimma include Agaro, Genet, Jimma, and Saqqa.</obo:IAO_0000115>
        <oboInOwl:hasOBONamespace>GAZ</oboInOwl:hasOBONamespace>
        <oboInOwl:id>GAZ:00031118</oboInOwl:id>
        <rdfs:label>Jimma Zone</rdfs:label>
    </owl:NamedIndividual>
    


    <!-- http://purl.obolibrary.org/obo/GAZ_00031119 -->

    <owl:NamedIndividual rdf:about="http://purl.obolibrary.org/obo/GAZ_00031119">
        <obo:RO_0001025 rdf:resource="http://purl.obolibrary.org/obo/GAZ_00000784"/>
        <obo:IAO_0000115>One of the 12 Zones of the Ethiopian Region of Oromia. Misraq Shewa is located in the middle of Oromia, connecting the western regions to the eastern ones. This zone is bordered on the south and southwest by the Southern Nations, Nationalities and Peoples Region, on the west by Mirab Shewa, on the northwest by Semien Shewa, on the north by the Amhara Region, on the northeast by the Afar Region, and on the southwest by Arsi; its westernmost reach is defined by the course of the Bilate River. Towns and cities in Misraq Shewa include Adama, Debre Zeit, Metehara, Shashamane, and Ziway.</obo:IAO_0000115>
        <oboInOwl:hasOBONamespace>GAZ</oboInOwl:hasOBONamespace>
        <oboInOwl:id>GAZ:00031119</oboInOwl:id>
        <rdfs:label>East Shewa Zone</rdfs:label>
    </owl:NamedIndividual>
    


    <!-- http://purl.obolibrary.org/obo/GAZ_00031120 -->

    <owl:NamedIndividual rdf:about="http://purl.obolibrary.org/obo/GAZ_00031120">
        <obo:RO_0001025 rdf:resource="http://purl.obolibrary.org/obo/GAZ_00000784"/>
        <obo:IAO_0000115>One of the 12 zones of the Oromia Region of Ethiopia. Illubabor is named for the former province Illubabor. Illubabor is bordered on the south by the Southern Nations, Nationalities and Peoples Region, on the southwest by the Gambela Region, on the west by Misraq Welega, on the north by the Benishangul-Gumuz Region, and on the east by Jimma. Towns and cities in Illubabor include Bedele, Gore and Metu.</obo:IAO_0000115>
        <oboInOwl:hasOBONamespace>GAZ</oboInOwl:hasOBONamespace>
        <oboInOwl:id>GAZ:00031120</oboInOwl:id>
        <rdfs:label>Illubabor Zone</rdfs:label>
    </owl:NamedIndividual>
    


    <!-- http://purl.obolibrary.org/obo/GAZ_00031121 -->

    <owl:NamedIndividual rdf:about="http://purl.obolibrary.org/obo/GAZ_00031121">
        <obo:RO_0001025 rdf:resource="http://purl.obolibrary.org/obo/GAZ_00000784"/>
        <obo:IAO_0000115>One of the 12 Zones in the Ethiopian Region of Oromia. Mirab Wellega is bordered on the south by the Gambela Region, on the west by Sudan, on the north by the Benishangul-Gumuz Region, on the east for a short space by Misraq Welega, and on the southeast by Illubabor. Its highest point is Mount Welel. Towns and cities in Mirab Welega include Dembidolo, Gimbi, Mendi, and Nejo.</obo:IAO_0000115>
        <oboInOwl:hasOBONamespace>GAZ</oboInOwl:hasOBONamespace>
        <oboInOwl:id>GAZ:00031121</oboInOwl:id>
        <rdfs:label>West Welega Zone</rdfs:label>
    </owl:NamedIndividual>
    


    <!-- http://purl.obolibrary.org/obo/GAZ_00031122 -->

    <owl:NamedIndividual rdf:about="http://purl.obolibrary.org/obo/GAZ_00031122">
        <obo:RO_0001025 rdf:resource="http://purl.obolibrary.org/obo/GAZ_00000784"/>
        <obo:IAO_0000115>One of the 12 Zones of the Ethiopian Region of Oromia. Semien Shewa is bordered on the south by Addis Ababa, on the southwest by Mirab Shewa, on the north by the Amhara Region, and on the southeast by Misraq Shewa. Towns and cities in Semien Shewa include Debre Libanos, Fiche and Gebre Guracha.</obo:IAO_0000115>
        <oboInOwl:hasOBONamespace>GAZ</oboInOwl:hasOBONamespace>
        <oboInOwl:id>GAZ:00031122</oboInOwl:id>
        <rdfs:label>North Shewa Zone</rdfs:label>
    </owl:NamedIndividual>
    


    <!-- http://purl.obolibrary.org/obo/GAZ_00031123 -->

    <owl:NamedIndividual rdf:about="http://purl.obolibrary.org/obo/GAZ_00031123">
        <obo:RO_0001025 rdf:resource="http://purl.obolibrary.org/obo/GAZ_00000784"/>
        <obo:IAO_0000115>One of the 12 Zones in the Ethiopian Region of Oromia. Misraq Welega is bounded on the southwest by Illubabor, on the west by the Didessa River which separates it from Mirab Welega, on the northwest and north by the Benishangul-Gumuz Region, on the east by Mirab Shewa, and on the southeast by Jimma. The highest point in this zone is Mount Garochan (3,276 m).</obo:IAO_0000115>
        <oboInOwl:hasOBONamespace>GAZ</oboInOwl:hasOBONamespace>
        <oboInOwl:id>GAZ:00031123</oboInOwl:id>
        <rdfs:label>East Welega Zone</rdfs:label>
    </owl:NamedIndividual>
    


    <!-- http://purl.obolibrary.org/obo/GAZ_00031124 -->

    <owl:NamedIndividual rdf:about="http://purl.obolibrary.org/obo/GAZ_00031124">
        <obo:RO_0001025 rdf:resource="http://purl.obolibrary.org/obo/GAZ_00000784"/>
        <obo:IAO_0000115>One of the 12 Zones in the Ethiopian Region of Oromia. Mirab Harerge is bordered on the south by the Shebelle River which separates it from Bale, on the southwest by Arsi, on the northwest by the Afar Region, on the north by the Somali Region and on the east by Misraq Hararghe. Towns in Mirab Hararghe include Asebe Teferi, Bedessa, Gelemso, and Mieso.</obo:IAO_0000115>
        <oboInOwl:hasOBONamespace>GAZ</oboInOwl:hasOBONamespace>
        <oboInOwl:id>GAZ:00031124</oboInOwl:id>
        <rdfs:label>West Harerge Zone</rdfs:label>
    </owl:NamedIndividual>
    


    <!-- http://purl.obolibrary.org/obo/GAZ_00031125 -->

    <owl:NamedIndividual rdf:about="http://purl.obolibrary.org/obo/GAZ_00031125">
        <obo:RO_0001025 rdf:resource="http://purl.obolibrary.org/obo/GAZ_00000784"/>
        <obo:IAO_0000115>One of the 12 zones of the Oromia Region in Ethiopia. Mirab Shewa is bordered on the south by the Southern Nations, Nationalities and Peoples Region, on the southwest by Jimma, on the northwest by Misraq Welega, on the north by the Amhara Region, on the northeast by Semien Shewa, and on the southeast by Misraq Shewa. Its highest point is Mount Wenchi. Towns and cities in Mirab Shewa include Alem Gena, Ambo, Holeta Genet and Waliso.</obo:IAO_0000115>
        <oboInOwl:hasOBONamespace>GAZ</oboInOwl:hasOBONamespace>
        <oboInOwl:id>GAZ:00031125</oboInOwl:id>
        <rdfs:label>West Shewa Zone</rdfs:label>
    </owl:NamedIndividual>
    


    <!-- http://purl.obolibrary.org/obo/GAZ_00031126 -->

    <owl:NamedIndividual rdf:about="http://purl.obolibrary.org/obo/GAZ_00031126">
        <obo:RO_0001025 rdf:resource="http://purl.obolibrary.org/obo/GAZ_00000785"/>
        <obo:IAO_0000115>One of the nine Zones of the Somali Region of Ethiopia. Liben is bordered on the south by Kenya, on the west by the Oromia Region, on the northeast by Afder, and on the southeast by Somalia. Towns and cities in Liben include Softu and Dolo.</obo:IAO_0000115>
        <oboInOwl:hasOBONamespace>GAZ</oboInOwl:hasOBONamespace>
        <oboInOwl:id>GAZ:00031126</oboInOwl:id>
        <rdfs:label>Liben Zone</rdfs:label>
    </owl:NamedIndividual>
    


    <!-- http://purl.obolibrary.org/obo/GAZ_00031127 -->

    <owl:NamedIndividual rdf:about="http://purl.obolibrary.org/obo/GAZ_00031127">
        <obo:RO_0001025 rdf:resource="http://purl.obolibrary.org/obo/GAZ_00000785"/>
        <obo:IAO_0000115>One of nine Zones of the Somali Region of Ethiopia. Afder is bordered on the southwest by the Ganale Dorya River which separates it from Liben, on the west by the Oromia Region, on north and northeast by the Shebelle River separates it from Gode, and on the east and southeast by Somalia. Towns and cities in Afder include Cherti and Weldiya.</obo:IAO_0000115>
        <oboInOwl:hasOBONamespace>GAZ</oboInOwl:hasOBONamespace>
        <oboInOwl:id>GAZ:00031127</oboInOwl:id>
        <rdfs:label>Afder Zone</rdfs:label>
    </owl:NamedIndividual>
    


    <!-- http://purl.obolibrary.org/obo/GAZ_00031128 -->

    <owl:NamedIndividual rdf:about="http://purl.obolibrary.org/obo/GAZ_00031128">
        <obo:RO_0001025 rdf:resource="http://purl.obolibrary.org/obo/GAZ_00000785"/>
        <obo:IAO_0000115>One of nine Zones of the Ethiopian Somali Region. Shinile is named for its largest town, Shinile. Located at the northwestern point of the Somali Region, and stretching across the savanna north of the Amhar mountains, Shinile is bordered on the south by the Oromia Region, on the west by the Afar Region, on the north by Djibouti, and on the east by Jijiga.</obo:IAO_0000115>
        <oboInOwl:hasOBONamespace>GAZ</oboInOwl:hasOBONamespace>
        <oboInOwl:id>GAZ:00031128</oboInOwl:id>
        <rdfs:label>Shinile Zone</rdfs:label>
    </owl:NamedIndividual>
    


    <!-- http://purl.obolibrary.org/obo/GAZ_00031129 -->

    <owl:NamedIndividual rdf:about="http://purl.obolibrary.org/obo/GAZ_00031129">
        <obo:RO_0001025 rdf:resource="http://purl.obolibrary.org/obo/GAZ_00000785"/>
        <obo:IAO_0000115>One of the nine Zones in the Somali Region of Ethiopia. Deghabur is bordered on the south by Korahe and Gode, on the west by Fiq, on the northwest by the Oromia Region, on the north by Jijiga and Somalia, and on the east by Werder.</obo:IAO_0000115>
        <oboInOwl:hasOBONamespace>GAZ</oboInOwl:hasOBONamespace>
        <oboInOwl:id>GAZ:00031129</oboInOwl:id>
        <rdfs:label>Degehabur Zone</rdfs:label>
    </owl:NamedIndividual>
    


    <!-- http://purl.obolibrary.org/obo/GAZ_00031130 -->

    <owl:NamedIndividual rdf:about="http://purl.obolibrary.org/obo/GAZ_00031130">
        <obo:RO_0001025 rdf:resource="http://purl.obolibrary.org/obo/GAZ_00000785"/>
        <obo:IAO_0000115>One of nine Zones of the Somali Region of Ethiopia. Korahe is bordered on the south and west by Gode, on the north by Degehabur, and on the east by Werder. The largest city in Korahe is Kebri Dahar.</obo:IAO_0000115>
        <oboInOwl:hasOBONamespace>GAZ</oboInOwl:hasOBONamespace>
        <oboInOwl:id>GAZ:00031130</oboInOwl:id>
        <rdfs:label>Korahe Zone</rdfs:label>
    </owl:NamedIndividual>
    


    <!-- http://purl.obolibrary.org/obo/GAZ_00031131 -->

    <owl:NamedIndividual rdf:about="http://purl.obolibrary.org/obo/GAZ_00031131">
        <obo:RO_0001025 rdf:resource="http://purl.obolibrary.org/obo/GAZ_00000785"/>
        <obo:IAO_0000115>One of nine zones of the Ethiopian Somali Region. Other towns and cities in this zone include Awbere, Derwonaji and Hart Sheik. Jijiga is bordered on the south by Degehabur, on the west by the Oromia Region, on the north by Shinile and on the east by Somalia.</obo:IAO_0000115>
        <oboInOwl:hasOBONamespace>GAZ</oboInOwl:hasOBONamespace>
        <oboInOwl:id>GAZ:00031131</oboInOwl:id>
        <rdfs:label>Jigjiga Zone</rdfs:label>
    </owl:NamedIndividual>
    


    <!-- http://purl.obolibrary.org/obo/GAZ_00031132 -->

    <owl:NamedIndividual rdf:about="http://purl.obolibrary.org/obo/GAZ_00031132">
        <obo:RO_0001025 rdf:resource="http://purl.obolibrary.org/obo/GAZ_00000785"/>
        <obo:IAO_0000115>One of nine Zones of the Somali Region in Ethiopia. Werder is bordered on the south by Gode, on the west by Korahe, on the northwest by Degehabur, and on the northeast and southeast by Somalia.</obo:IAO_0000115>
        <oboInOwl:hasOBONamespace>GAZ</oboInOwl:hasOBONamespace>
        <oboInOwl:id>GAZ:00031132</oboInOwl:id>
        <rdfs:label>Warder Zone</rdfs:label>
    </owl:NamedIndividual>
    


    <!-- http://purl.obolibrary.org/obo/GAZ_00031133 -->

    <owl:NamedIndividual rdf:about="http://purl.obolibrary.org/obo/GAZ_00031133">
        <obo:RO_0001025 rdf:resource="http://purl.obolibrary.org/obo/GAZ_00000785"/>
        <obo:IAO_0000115>One of nine Zones of the Somali Region of Ethiopia. Gode is bordered on the south by Afder, on the west by the Oromia Region, on the north by Fiq and Degehabur, on the northeast by Korahe and Werder, and on the east by Somalia. The Shebelle River defines its southern and western boundaries.</obo:IAO_0000115>
        <oboInOwl:hasOBONamespace>GAZ</oboInOwl:hasOBONamespace>
        <oboInOwl:id>GAZ:00031133</oboInOwl:id>
        <rdfs:label>Gode Zone</rdfs:label>
    </owl:NamedIndividual>
    


    <!-- http://purl.obolibrary.org/obo/GAZ_00031134 -->

    <owl:NamedIndividual rdf:about="http://purl.obolibrary.org/obo/GAZ_00031134">
        <obo:RO_0001025 rdf:resource="http://purl.obolibrary.org/obo/GAZ_00000786"/>
        <obo:IAO_0000115>A Zone in the Ethiopian Southern Nations, Nationalities and Peoples Region (SNNPR). Keficho Shekicho is bordered on the south by Debub Omo, on the southwest by Bench Maji, on the west and north by the Oromia Region, and on the east by Semien Omo. The administrative center of Keficho Shekicho is Bonga; other towns include Tippi.</obo:IAO_0000115>
        <oboInOwl:hasOBONamespace>GAZ</oboInOwl:hasOBONamespace>
        <oboInOwl:id>GAZ:00031134</oboInOwl:id>
        <rdfs:label>Keficho Shekicho Zone</rdfs:label>
    </owl:NamedIndividual>
    


    <!-- http://purl.obolibrary.org/obo/GAZ_00031135 -->

    <owl:NamedIndividual rdf:about="http://purl.obolibrary.org/obo/GAZ_00031135">
        <obo:RO_0001025 rdf:resource="http://purl.obolibrary.org/obo/GAZ_00000786"/>
        <obo:IAO_0000115>A Zone in the Ethiopian Southern Nations, Nationalities and Peoples Region (SNNPR). Hadiya is bordered on the south by Kembata Alaba and Tembaro (KAT), on the west by the Omo River which separates it from Oromia Region and the Yem Special Woreda, on the north by Gurage, and on the east by the Oromia Region; the woreda of Badawacho is an exclave separated from the rest of the zone by the KAT. The administrative center of Hadiya is Hosaena.</obo:IAO_0000115>
        <oboInOwl:hasOBONamespace>GAZ</oboInOwl:hasOBONamespace>
        <oboInOwl:id>GAZ:00031135</oboInOwl:id>
        <rdfs:label>Hadiya Zone</rdfs:label>
    </owl:NamedIndividual>
    


    <!-- http://purl.obolibrary.org/obo/GAZ_00031136 -->

    <owl:NamedIndividual rdf:about="http://purl.obolibrary.org/obo/GAZ_00031136">
        <obo:RO_0001025 rdf:resource="http://purl.obolibrary.org/obo/GAZ_00000786"/>
        <obo:IAO_0000115>A Zone in the Southern Nations, Nationalities and Peoples Region (SNNPR) of Ethiopia. Gedeo is bordered on the east, south and west by the Oromia Region, and on the north by Sidama. Dila is the administrative center; other towns include Yirgachefe.</obo:IAO_0000115>
        <oboInOwl:hasOBONamespace>GAZ</oboInOwl:hasOBONamespace>
        <oboInOwl:id>GAZ:00031136</oboInOwl:id>
        <rdfs:label>Gedeo Zone</rdfs:label>
    </owl:NamedIndividual>
    


    <!-- http://purl.obolibrary.org/obo/GAZ_00031138 -->

    <owl:NamedIndividual rdf:about="http://purl.obolibrary.org/obo/GAZ_00031138">
        <obo:RO_0001025 rdf:resource="http://purl.obolibrary.org/obo/GAZ_00000786"/>
        <obo:IAO_0000115>One of the 79 woredas in the Southern Nations, Nationalities, and Peoples Region (SNNPR) of Ethiopia. Because Burji is not part of any Zone in the SNNPR, it is considered a Special woreda. Burji is bordered on the east and south by the Oromia Region, on the west by the Konso Special Woreda, and on the north by the Amaro Special Woreda. The administrative center of Burji is Soyama.</obo:IAO_0000115>
        <oboInOwl:hasOBONamespace>GAZ</oboInOwl:hasOBONamespace>
        <oboInOwl:id>GAZ:00031138</oboInOwl:id>
        <rdfs:label>Burji Special Woreda</rdfs:label>
    </owl:NamedIndividual>
    


    <!-- http://purl.obolibrary.org/obo/GAZ_00031139 -->

    <owl:NamedIndividual rdf:about="http://purl.obolibrary.org/obo/GAZ_00031139">
        <obo:RO_0001025 rdf:resource="http://purl.obolibrary.org/obo/GAZ_00000786"/>
        <obo:IAO_0000115>A Zone in the Ethiopian Southern Nations, Nationalities and Peoples Region (SNNPR). Sidama is bordered on the south by the Oromia Region except for a short stretch in the middle where it shares a border with Gedeo, on the west by the Bilate River which separates it from Semien Omo, and on the north and east by the Oromia Region. The administrative center for Sidama is Awasa; other towns include Awasa, Irgalem, and Wendo.</obo:IAO_0000115>
        <oboInOwl:hasOBONamespace>GAZ</oboInOwl:hasOBONamespace>
        <oboInOwl:id>GAZ:00031139</oboInOwl:id>
        <rdfs:label>Sidama Zone</rdfs:label>
    </owl:NamedIndividual>
    


    <!-- http://purl.obolibrary.org/obo/GAZ_00031140 -->

    <owl:NamedIndividual rdf:about="http://purl.obolibrary.org/obo/GAZ_00031140">
        <obo:RO_0001025 rdf:resource="http://purl.obolibrary.org/obo/GAZ_00000786"/>
        <obo:IAO_0000115>One of the 79 woredas in the Southern Nations, Nationalities, and Peoples Region (SNNPR) of Ethiopia. Because Yem is not part of any Zone in the SNNPR, it is considered a Special woreda. Yem is bordered on the west by the Oromia Region, and separated from Gurage on the northeast and Hadiya on the east by the Omo River. The administrative center of Yem is Fofa.</obo:IAO_0000115>
        <oboInOwl:hasOBONamespace>GAZ</oboInOwl:hasOBONamespace>
        <oboInOwl:id>GAZ:00031140</oboInOwl:id>
        <rdfs:label>Yem Special Woreda</rdfs:label>
    </owl:NamedIndividual>
    


    <!-- http://purl.obolibrary.org/obo/GAZ_00031141 -->

    <owl:NamedIndividual rdf:about="http://purl.obolibrary.org/obo/GAZ_00031141">
        <obo:RO_0001025 rdf:resource="http://purl.obolibrary.org/obo/GAZ_00000786"/>
        <obo:IAO_0000115>A Zone in the Ethiopian Southern Nations, Nationalities and Peoples Region (SNNPR). KAT is bordered on the south by Semien Omo, on the northwest by Hadiya, on the north by Gurage, on the east by the Oromia Region, and on the southeast by Badawacho, an exclave of the Hadiya Zone. The administrative center of KAT is Durame; other important towns include Alaba Kulito and Shinshicho. Other local landmarks include the three mountains of Ambaricho, Kataa, and Datoo, and the hot springs at Motokoma. The longest river in the area is the Lagabora which means in Kambatinga the &quot;river of Bora&quot;.</obo:IAO_0000115>
        <oboInOwl:hasOBONamespace>GAZ</oboInOwl:hasOBONamespace>
        <oboInOwl:id>GAZ:00031141</oboInOwl:id>
        <rdfs:label>Kembata Alaba and Tembaro Zone</rdfs:label>
    </owl:NamedIndividual>
    


    <!-- http://purl.obolibrary.org/obo/GAZ_00031142 -->

    <owl:NamedIndividual rdf:about="http://purl.obolibrary.org/obo/GAZ_00031142">
        <obo:RO_0001025 rdf:resource="http://purl.obolibrary.org/obo/GAZ_00000786"/>
        <obo:IAO_0000115>Dirashe is one of the 77 woredas in the Southern Nations, Nationalities, and Peoples Region (SNNPR) of Ethiopia. Because Dirashe is not part of any Zone in the SNNPR, it is considered a Special woreda. Located in the Great Rift Valley, Dirashe is bordered on the south by Konso special woreda, on the west by the Weito River which separates it from the Debub Omo Zone, on the north by the Semien Omo Zone, on the northeast by Lake Chamo, and on the east by Amaro special woreda. The administrative center of Dirashe is Gidole.</obo:IAO_0000115>
        <oboInOwl:hasOBONamespace>GAZ</oboInOwl:hasOBONamespace>
        <oboInOwl:id>GAZ:00031142</oboInOwl:id>
        <rdfs:label>Dirashe Special Woreda</rdfs:label>
    </owl:NamedIndividual>
    


    <!-- http://purl.obolibrary.org/obo/GAZ_00031143 -->

    <owl:NamedIndividual rdf:about="http://purl.obolibrary.org/obo/GAZ_00031143">
        <obo:RO_0001025 rdf:resource="http://purl.obolibrary.org/obo/GAZ_00000786"/>
        <obo:IAO_0000115>A Zone in the Ethiopian Southern Nations, Nationalities and Peoples Region (SNNPR). Debub Omo is bordered on the south by Kenya, on the southwest by the Ilemi Triangle, on the west by Bench Maji, on the northwest by Keficho Shekicho, on the north by Semien Omo, on the northeast by the Dirashe and Konso Special Woredas, and on the east by the Oromia Region. The administrative center of Debub Omo is Jinka.</obo:IAO_0000115>
        <oboInOwl:hasOBONamespace>GAZ</oboInOwl:hasOBONamespace>
        <oboInOwl:id>GAZ:00031143</oboInOwl:id>
        <rdfs:label>South Omo Zone</rdfs:label>
    </owl:NamedIndividual>
    


    <!-- http://purl.obolibrary.org/obo/GAZ_00031144 -->

    <owl:NamedIndividual rdf:about="http://purl.obolibrary.org/obo/GAZ_00031144">
        <obo:RO_0001025 rdf:resource="http://purl.obolibrary.org/obo/GAZ_00000786"/>
        <obo:IAO_0000115>One of the 79 woredas in the Southern Nations, Nationalities, and Peoples Region (SNNPR) of Ethiopia. Because Amaro is not part of any Zone in the SNNPR, it is considered a Special woreda. Located in the Great Rift Valley, Amaro is bordered on the south by Burji Special Woreda, on the east by Semien Omo and Lake Chamo, and on the north and east by the Oromia Region. It is divided into 32 kebeles. The administrative center of the woreda is Kele.</obo:IAO_0000115>
        <oboInOwl:hasOBONamespace>GAZ</oboInOwl:hasOBONamespace>
        <oboInOwl:id>GAZ:00031144</oboInOwl:id>
        <rdfs:label>Amaro Special Woreda</rdfs:label>
    </owl:NamedIndividual>
    


    <!-- http://purl.obolibrary.org/obo/GAZ_00031145 -->

    <owl:NamedIndividual rdf:about="http://purl.obolibrary.org/obo/GAZ_00031145">
        <obo:RO_0001025 rdf:resource="http://purl.obolibrary.org/obo/GAZ_00000786"/>
        <obo:IAO_0000115>A Zone in the Ethiopian Southern Nations, Nationalities and Peoples Region (SNNPR). This zone is named for the Omo River, which flows in its western area. While in their latest population estimates the Central Statistical Agency (CSA) includes it as a single Zone, the list of second administrative level bodies maintained by the United Nations Geographic Information Working Group divides it into two, Dawro and Gamo Goffa, and categorizes Basketo as a special woreda. Semien Omo is bordered on the south by Debub Omo, on the west by Keficho Shekicho, on the northwest by the Oromia Region, on the north by Kembata Alaba and Tembaro, on the northeast by part of the Oromia Region, on the east by the Bilate River which separates it from Sidama and another part of the Oromia Region, and on the southeast by the Amaro and Dirashe Special Woredas. The highest point in Semien Omo is Mount Gurage, northwest of Chencha, and this mountain is also the highest summit (3719 m) in the SNNPR.</obo:IAO_0000115>
        <oboInOwl:hasOBONamespace>GAZ</oboInOwl:hasOBONamespace>
        <oboInOwl:id>GAZ:00031145</oboInOwl:id>
        <rdfs:label>North Omo Zone</rdfs:label>
    </owl:NamedIndividual>
    


    <!-- http://purl.obolibrary.org/obo/GAZ_00031146 -->

    <owl:NamedIndividual rdf:about="http://purl.obolibrary.org/obo/GAZ_00031146">
        <obo:RO_0001025 rdf:resource="http://purl.obolibrary.org/obo/GAZ_00000786"/>
        <obo:IAO_0000115>A Zone in the Ethiopian Southern Nations, Nationalities and Peoples Region (SNNPR). Gurage is bordered on the south by Hadiya on the west north and east by the Oromia Region, and on the southeast by Kembata Alaba and Tembaro (KAT). Its highest point is Mount Gurage. Welkite is the administrative center of the Zone; other towns in Gurage include Butajira and Worabe.</obo:IAO_0000115>
        <oboInOwl:hasOBONamespace>GAZ</oboInOwl:hasOBONamespace>
        <oboInOwl:id>GAZ:00031146</oboInOwl:id>
        <rdfs:label>Gurage Zone</rdfs:label>
    </owl:NamedIndividual>
    


    <!-- http://purl.obolibrary.org/obo/GAZ_00031147 -->

    <owl:NamedIndividual rdf:about="http://purl.obolibrary.org/obo/GAZ_00031147">
        <obo:RO_0001025 rdf:resource="http://purl.obolibrary.org/obo/GAZ_00000786"/>
        <obo:IAO_0000115>A Zone in the Ethiopian Southern Nations, Nationalities and Peoples Region (SNNPR). Bench Maji is bordered on the south by the Ilemi Triangle, on the west by Sudan, on the northwest by the Gambela Region, on the north by Keficho Shekicho and on the east by Debub Omo.</obo:IAO_0000115>
        <oboInOwl:hasOBONamespace>GAZ</oboInOwl:hasOBONamespace>
        <oboInOwl:id>GAZ:00031147</oboInOwl:id>
        <rdfs:label>Bench Maji Zone</rdfs:label>
    </owl:NamedIndividual>
    


    <!-- http://purl.obolibrary.org/obo/GAZ_00031148 -->

    <owl:NamedIndividual rdf:about="http://purl.obolibrary.org/obo/GAZ_00031148">
        <obo:RO_0001025 rdf:resource="http://purl.obolibrary.org/obo/GAZ_00000787"/>
        <obo:IAO_0000115>A Zone in the Ethiopian Region of Tigray. Mehakelegnaw is bordered on the east by Misraqawi (Eastern), on the south by Debubawi (Southern), on the west by Mirabawi (Western) and on the north by Eritrea. Towns and cities in Mehakelegnaw include Axum and Adwa, as well as the historically significant village of Yeha and the ancient monastery of Debre Damo.</obo:IAO_0000115>
        <oboInOwl:hasOBONamespace>GAZ</oboInOwl:hasOBONamespace>
        <oboInOwl:id>GAZ:00031148</oboInOwl:id>
        <rdfs:label>Central Tigray Zone</rdfs:label>
    </owl:NamedIndividual>
    


    <!-- http://purl.obolibrary.org/obo/GAZ_00031149 -->

    <owl:NamedIndividual rdf:about="http://purl.obolibrary.org/obo/GAZ_00031149">
        <obo:RO_0001025 rdf:resource="http://purl.obolibrary.org/obo/GAZ_00000787"/>
        <obo:IAO_0000115>One of five Zones in the Ethiopian Region of Tigray. Debubawi is bordered on the south and west by the Amhara Region, on the northwest by Mehakelegnaw (Central), the north by Misraqawi (Eastern) and on the east by the Afar Region. Its highest point is Mount Alage. Towns and cities in Debubawi include Alamata, and Mek&apos;ele.</obo:IAO_0000115>
        <oboInOwl:hasOBONamespace>GAZ</oboInOwl:hasOBONamespace>
        <oboInOwl:id>GAZ:00031149</oboInOwl:id>
        <rdfs:label>South Tigray Zone</rdfs:label>
    </owl:NamedIndividual>
    


    <!-- http://purl.obolibrary.org/obo/GAZ_00031150 -->

    <owl:NamedIndividual rdf:about="http://purl.obolibrary.org/obo/GAZ_00031150">
        <obo:RO_0001025 rdf:resource="http://purl.obolibrary.org/obo/GAZ_00031149"/>
        <obo:IAO_0000115>A woreda in northern Ethiopia. Located in Enderta which is in the Debubawi Zone, Mekele is the capital of the Tigray Region. An enclave within Enderta Woreda.</obo:IAO_0000115>
        <oboInOwl:hasOBONamespace>GAZ</oboInOwl:hasOBONamespace>
        <oboInOwl:id>GAZ:00031150</oboInOwl:id>
        <rdfs:label>Mekele Woreda</rdfs:label>
    </owl:NamedIndividual>
    


    <!-- http://purl.obolibrary.org/obo/GAZ_00031151 -->

    <owl:NamedIndividual rdf:about="http://purl.obolibrary.org/obo/GAZ_00031151">
        <obo:RO_0001025 rdf:resource="http://purl.obolibrary.org/obo/GAZ_00000787"/>
        <obo:IAO_0000115>A Zone in the Ethiopian Region of Tigray. Misraqawi is bordered on the east by the Afar Region, on the south by Debubawi (Southern), on the west by Mehakelegnaw (Central) and on the north by Eritrea. Its highest point is Mount Asimba (3,250 m). Towns and cities in Misraqawi include Adigrat, Atsbi, Hawzen, and Wiqro.</obo:IAO_0000115>
        <oboInOwl:hasOBONamespace>GAZ</oboInOwl:hasOBONamespace>
        <oboInOwl:id>GAZ:00031151</oboInOwl:id>
        <rdfs:label>East Tigray Zone</rdfs:label>
    </owl:NamedIndividual>
    


    <!-- http://purl.obolibrary.org/obo/GAZ_00031152 -->

    <owl:NamedIndividual rdf:about="http://purl.obolibrary.org/obo/GAZ_00031152">
        <obo:RO_0001025 rdf:resource="http://purl.obolibrary.org/obo/GAZ_00000787"/>
        <obo:IAO_0000115>One of four Zones in the Ethiopian Tigray Region. Mi&apos;irabawi is bordered on the east by the Mehakelegnaw (Central) Zone, the south by the Amhara Region, the west by Sudan and on the north by Eritrea. Major towns and cities in this zone include Badme, Dima, Humera and Inda Selassie.</obo:IAO_0000115>
        <oboInOwl:hasOBONamespace>GAZ</oboInOwl:hasOBONamespace>
        <oboInOwl:id>GAZ:00031152</oboInOwl:id>
        <rdfs:label>West Tigray Zone</rdfs:label>
    </owl:NamedIndividual>
    


    <!-- http://purl.obolibrary.org/obo/GAZ_00040045 -->

    <owl:NamedIndividual rdf:about="http://purl.obolibrary.org/obo/GAZ_00040045">
        <obo:RO_0001025 rdf:resource="http://purl.obolibrary.org/obo/GAZ_00015452"/>
        <obo:IAO_0000115>An archipelago of eighty-four islands in the northwest of Lake Victoria, Uganda. The islands lie in two main groups, separated by the Kkome Channel.</obo:IAO_0000115>
        <oboInOwl:hasOBONamespace>GAZ</oboInOwl:hasOBONamespace>
        <oboInOwl:id>GAZ:00040045</oboInOwl:id>
        <rdfs:label>Ssese Islands</rdfs:label>
    </owl:NamedIndividual>
    


    <!-- http://purl.obolibrary.org/obo/GAZ_00040046 -->

    <owl:NamedIndividual rdf:about="http://purl.obolibrary.org/obo/GAZ_00040046">
        <obo:RO_0001025 rdf:resource="http://purl.obolibrary.org/obo/GAZ_00040045"/>
        <oboInOwl:hasOBONamespace>GAZ</oboInOwl:hasOBONamespace>
        <oboInOwl:id>GAZ:00040046</oboInOwl:id>
        <rdfs:label>Northeast Ssese Islands</rdfs:label>
    </owl:NamedIndividual>
    


    <!-- http://purl.obolibrary.org/obo/GAZ_00040047 -->

    <owl:NamedIndividual rdf:about="http://purl.obolibrary.org/obo/GAZ_00040047">
        <obo:RO_0001025 rdf:resource="http://purl.obolibrary.org/obo/GAZ_00040045"/>
        <oboInOwl:hasOBONamespace>GAZ</oboInOwl:hasOBONamespace>
        <oboInOwl:id>GAZ:00040047</oboInOwl:id>
        <rdfs:label>Southwest Ssese Islands</rdfs:label>
    </owl:NamedIndividual>
    


    <!-- http://purl.obolibrary.org/obo/GAZ_00040048 -->

    <owl:NamedIndividual rdf:about="http://purl.obolibrary.org/obo/GAZ_00040048">
        <obo:RO_0001025 rdf:resource="http://purl.obolibrary.org/obo/GAZ_00040046"/>
        <oboInOwl:hasOBONamespace>GAZ</oboInOwl:hasOBONamespace>
        <oboInOwl:id>GAZ:00040048</oboInOwl:id>
        <rdfs:label>Damba Island</rdfs:label>
    </owl:NamedIndividual>
    


    <!-- http://purl.obolibrary.org/obo/GAZ_00040049 -->

    <owl:NamedIndividual rdf:about="http://purl.obolibrary.org/obo/GAZ_00040049">
        <obo:RO_0001025 rdf:resource="http://purl.obolibrary.org/obo/GAZ_00040046"/>
        <oboInOwl:hasOBONamespace>GAZ</oboInOwl:hasOBONamespace>
        <oboInOwl:id>GAZ:00040049</oboInOwl:id>
        <rdfs:label>Kkome Island</rdfs:label>
    </owl:NamedIndividual>
    


    <!-- http://purl.obolibrary.org/obo/GAZ_00040050 -->

    <owl:NamedIndividual rdf:about="http://purl.obolibrary.org/obo/GAZ_00040050">
        <obo:RO_0001025 rdf:resource="http://purl.obolibrary.org/obo/GAZ_00040046"/>
        <oboInOwl:hasOBONamespace>GAZ</oboInOwl:hasOBONamespace>
        <oboInOwl:id>GAZ:00040050</oboInOwl:id>
        <rdfs:label>Luwaji Island</rdfs:label>
    </owl:NamedIndividual>
    


    <!-- http://purl.obolibrary.org/obo/GAZ_00040051 -->

    <owl:NamedIndividual rdf:about="http://purl.obolibrary.org/obo/GAZ_00040051">
        <obo:RO_0001025 rdf:resource="http://purl.obolibrary.org/obo/GAZ_00040047"/>
        <oboInOwl:hasOBONamespace>GAZ</oboInOwl:hasOBONamespace>
        <oboInOwl:id>GAZ:00040051</oboInOwl:id>
        <rdfs:label>Buyova Island</rdfs:label>
    </owl:NamedIndividual>
    


    <!-- http://purl.obolibrary.org/obo/GAZ_00040052 -->

    <owl:NamedIndividual rdf:about="http://purl.obolibrary.org/obo/GAZ_00040052">
        <obo:RO_0001025 rdf:resource="http://purl.obolibrary.org/obo/GAZ_00040047"/>
        <oboInOwl:hasOBONamespace>GAZ</oboInOwl:hasOBONamespace>
        <oboInOwl:id>GAZ:00040052</oboInOwl:id>
        <rdfs:label>Serinya Island</rdfs:label>
    </owl:NamedIndividual>
    


    <!-- http://purl.obolibrary.org/obo/GAZ_00040053 -->

    <owl:NamedIndividual rdf:about="http://purl.obolibrary.org/obo/GAZ_00040053">
        <obo:RO_0001025 rdf:resource="http://purl.obolibrary.org/obo/GAZ_00040047"/>
        <oboInOwl:hasOBONamespace>GAZ</oboInOwl:hasOBONamespace>
        <oboInOwl:id>GAZ:00040053</oboInOwl:id>
        <rdfs:label>Funve Island</rdfs:label>
    </owl:NamedIndividual>
    


    <!-- http://purl.obolibrary.org/obo/GAZ_00040054 -->

    <owl:NamedIndividual rdf:about="http://purl.obolibrary.org/obo/GAZ_00040054">
        <obo:RO_0001025 rdf:resource="http://purl.obolibrary.org/obo/GAZ_00040047"/>
        <obo:IAO_0000115>The second largest island in Lake Victoria, Uganda, after Ukerewe. Its area is 275 km2. It is a part of the Ssese Islands in the Kalangala District. Chief town is Kalangala.</obo:IAO_0000115>
        <oboInOwl:hasOBONamespace>GAZ</oboInOwl:hasOBONamespace>
        <oboInOwl:id>GAZ:00040054</oboInOwl:id>
        <rdfs:label>Bugala Island</rdfs:label>
    </owl:NamedIndividual>
    


    <!-- http://purl.obolibrary.org/obo/GAZ_00040055 -->

    <owl:NamedIndividual rdf:about="http://purl.obolibrary.org/obo/GAZ_00040055">
        <obo:RO_0001025 rdf:resource="http://purl.obolibrary.org/obo/GAZ_00040047"/>
        <oboInOwl:hasOBONamespace>GAZ</oboInOwl:hasOBONamespace>
        <oboInOwl:id>GAZ:00040055</oboInOwl:id>
        <rdfs:label>Bufumira Island</rdfs:label>
    </owl:NamedIndividual>
    


    <!-- http://purl.obolibrary.org/obo/GAZ_00040056 -->

    <owl:NamedIndividual rdf:about="http://purl.obolibrary.org/obo/GAZ_00040056">
        <obo:RO_0001025 rdf:resource="http://purl.obolibrary.org/obo/GAZ_00040047"/>
        <oboInOwl:hasOBONamespace>GAZ</oboInOwl:hasOBONamespace>
        <oboInOwl:id>GAZ:00040056</oboInOwl:id>
        <rdfs:label>Bukasa Island</rdfs:label>
    </owl:NamedIndividual>
    


    <!-- http://purl.obolibrary.org/obo/GAZ_00040057 -->

    <owl:NamedIndividual rdf:about="http://purl.obolibrary.org/obo/GAZ_00040057">
        <obo:RO_0001025 rdf:resource="http://purl.obolibrary.org/obo/GAZ_00040047"/>
        <oboInOwl:hasOBONamespace>GAZ</oboInOwl:hasOBONamespace>
        <oboInOwl:id>GAZ:00040057</oboInOwl:id>
        <rdfs:label>Bugaba Island</rdfs:label>
    </owl:NamedIndividual>
    


    <!-- http://purl.obolibrary.org/obo/GAZ_00040058 -->

    <owl:NamedIndividual rdf:about="http://purl.obolibrary.org/obo/GAZ_00040058">
        <obo:RO_0001025 rdf:resource="http://purl.obolibrary.org/obo/GAZ_00040047"/>
        <oboInOwl:hasOBONamespace>GAZ</oboInOwl:hasOBONamespace>
        <oboInOwl:id>GAZ:00040058</oboInOwl:id>
        <rdfs:label>Bubeke Island</rdfs:label>
    </owl:NamedIndividual>
    


    <!-- http://purl.obolibrary.org/obo/GAZ_00041527 -->

    <owl:NamedIndividual rdf:about="http://purl.obolibrary.org/obo/GAZ_00041527">
        <obo:RO_0001025 rdf:resource="http://purl.obolibrary.org/obo/GAZ_00015452"/>
        <obo:IAO_0000115>The largest island in Lake Victoria, the largest inland island in Africa. Located 45 km north of Mwanza.</obo:IAO_0000115>
        <oboInOwl:hasOBONamespace>GAZ</oboInOwl:hasOBONamespace>
        <oboInOwl:id>GAZ:00041527</oboInOwl:id>
        <rdfs:label>Ukerewe Island</rdfs:label>
    </owl:NamedIndividual>
    


    <!-- http://purl.obolibrary.org/obo/GAZ_00041528 -->

    <owl:NamedIndividual rdf:about="http://purl.obolibrary.org/obo/GAZ_00041528">
        <obo:RO_0001025 rdf:resource="http://purl.obolibrary.org/obo/GAZ_00000007"/>
        <obo:IAO_0000115>An endorheic lake, in western Zomba District of Malawi, near the border with Mozambique.</obo:IAO_0000115>
        <oboInOwl:hasOBONamespace>GAZ</oboInOwl:hasOBONamespace>
        <oboInOwl:id>GAZ:00041528</oboInOwl:id>
        <rdfs:label>Lake Chilwa</rdfs:label>
    </owl:NamedIndividual>
    


    <!-- http://purl.obolibrary.org/obo/GAZ_00041529 -->

    <owl:NamedIndividual rdf:about="http://purl.obolibrary.org/obo/GAZ_00041529">
        <obo:RO_0001025 rdf:resource="http://purl.obolibrary.org/obo/GAZ_00000007"/>
        <obo:IAO_0000115>A lake in southern part of Malawi, in the Southern Region.</obo:IAO_0000115>
        <oboInOwl:hasOBONamespace>GAZ</oboInOwl:hasOBONamespace>
        <oboInOwl:id>GAZ:00041529</oboInOwl:id>
        <rdfs:label>Lake Malombe</rdfs:label>
    </owl:NamedIndividual>
    


    <!-- http://purl.obolibrary.org/obo/GAZ_00041530 -->

    <owl:NamedIndividual rdf:about="http://purl.obolibrary.org/obo/GAZ_00041530">
        <obo:RO_0001025 rdf:resource="http://purl.obolibrary.org/obo/GAZ_00000007"/>
        <obo:IAO_0000115>A freshwater lake on the longest arm of Africa&apos;s second-longest river, the Congo. Located on the border between Zambia and Democratic Republic of the Congo, it makes up 110 km of the total length of the Congo, lying between its Luapula River (upstream) and Luvua River (downstream) segments. Mweru is mainly fed by the Luapula River, which comes in through swamps from the south, and the Kalungwishi River from the east. At its north end the lake is drained by the Luvua River, which flows in a northwesterly direction to join the Lualaba River and thence to the Congo.</obo:IAO_0000115>
        <oboInOwl:hasOBONamespace>GAZ</oboInOwl:hasOBONamespace>
        <oboInOwl:id>GAZ:00041530</oboInOwl:id>
        <rdfs:label>Lake Mweru</rdfs:label>
    </owl:NamedIndividual>
    


    <!-- http://purl.obolibrary.org/obo/GAZ_00041531 -->

    <owl:NamedIndividual rdf:about="http://purl.obolibrary.org/obo/GAZ_00041531">
        <obo:RO_0001025 rdf:resource="http://purl.obolibrary.org/obo/GAZ_00000007"/>
        <obo:IAO_0000115>An alkaline lake in southwestern Tanzania. It is divided into two basins by a central swamp zone, ranging from 5-20 km wide. It is fed by 17 rivers. Seven rivers enter the south basin and 10 discharge to the north basin.</obo:IAO_0000115>
        <oboInOwl:hasOBONamespace>GAZ</oboInOwl:hasOBONamespace>
        <oboInOwl:id>GAZ:00041531</oboInOwl:id>
        <rdfs:label>Lake Rukwa</rdfs:label>
    </owl:NamedIndividual>
    


    <!-- http://purl.obolibrary.org/obo/GAZ_00041532 -->

    <owl:NamedIndividual rdf:about="http://purl.obolibrary.org/obo/GAZ_00041532">
        <obo:RO_0001025 rdf:resource="http://purl.obolibrary.org/obo/GAZ_00000007"/>
        <obo:IAO_0000115>An endorheic lake and swamp system in the Northern Province of Zambia. A rift valley lake lying in a branch of the Great Rift Valley, running from the Luapula River to Lake Tanganyika. There are some hot springs characteristics of a rift valley to the east. Its water is muddy in appearance, at times appearing reddish and &apos;slightly oily&apos;.</obo:IAO_0000115>
        <oboInOwl:hasOBONamespace>GAZ</oboInOwl:hasOBONamespace>
        <oboInOwl:id>GAZ:00041532</oboInOwl:id>
        <rdfs:label>Lake Mweru Wantipa</rdfs:label>
    </owl:NamedIndividual>
    


    <!-- http://purl.obolibrary.org/obo/GAZ_00041533 -->

    <owl:NamedIndividual rdf:about="http://purl.obolibrary.org/obo/GAZ_00041533">
        <obo:RO_0001025 rdf:resource="http://purl.obolibrary.org/obo/GAZ_00000007"/>
        <obo:IAO_0000115>A lake located in the western Great Rift Valley, on the border between the Democratic Republic of the Congo and Uganda, with its northern shore a few km south of the Equator. Lake Edward lies at an elevation of 920 metres, is 77 km long by 40 km wide at its maximum points, and covers a total surface area of 2,325 km2 (the 15th largest on the continent). The lake is fed by the Nyamugasani, the Ishasha, the Rutshuru, and the Rwindi rivers. It empties to the north via the Semliki River into Lake Albert. Lake George to the northeast empties into Lake Edward via the Kazinga Channel.</obo:IAO_0000115>
        <oboInOwl:hasOBONamespace>GAZ</oboInOwl:hasOBONamespace>
        <oboInOwl:id>GAZ:00041533</oboInOwl:id>
        <rdfs:label>Lake Edward</rdfs:label>
    </owl:NamedIndividual>
    


    <!-- http://purl.obolibrary.org/obo/GAZ_00041534 -->

    <owl:NamedIndividual rdf:about="http://purl.obolibrary.org/obo/GAZ_00041534">
        <obo:RO_0001025 rdf:resource="http://purl.obolibrary.org/obo/GAZ_00000007"/>
        <obo:IAO_0000115>A monomictic freshwater lake located in the center of the continent, on the border between Uganda and the Democratic Republic of the Congo (formerly Zaire). Lake Albert is the northernmost of the chain of lakes in the Great Rift Valley; it is about 160 km long and 30 km wide, with a maximum depth of 51 m, and a surface elevation of 619 m above sea level. Lake Albert is part of the complicated system of the upper Nile. Its main sources are the Victoria Nile, ultimately coming from Lake Victoria to the southeast, and the Semliki River, which issues from Lake Edward to the southwest. The water of the Victoria Nile is much less saline than that of Lake Albert. Its outlet, at the northernmost tip of the lake, is the Albert Nile (which becomes known as the Mountain Nile when it enters Sudan).</obo:IAO_0000115>
        <oboInOwl:hasOBONamespace>GAZ</oboInOwl:hasOBONamespace>
        <oboInOwl:id>GAZ:00041534</oboInOwl:id>
        <rdfs:label>Lake Albert</rdfs:label>
    </owl:NamedIndividual>
    


    <!-- http://purl.obolibrary.org/obo/GAZ_00041535 -->

    <owl:NamedIndividual rdf:about="http://purl.obolibrary.org/obo/GAZ_00041535">
        <rdf:type rdf:resource="http://purl.obolibrary.org/obo/ENVO_00000019"/>
        <obo:RO_0001025 rdf:resource="http://purl.obolibrary.org/obo/GAZ_00000007"/>
        <obo:IAO_0000115>A soda lake located in northern Tanzania, close to the Kenyan border, in Africa&apos;s Great Rift Valley. The lake is quite shallow, less than three m deep, and varies in width depending on its water level.</obo:IAO_0000115>
        <oboInOwl:hasOBONamespace>GAZ</oboInOwl:hasOBONamespace>
        <oboInOwl:id>GAZ:00041535</oboInOwl:id>
        <rdfs:label>Lake Natron</rdfs:label>
    </owl:NamedIndividual>
    


    <!-- http://purl.obolibrary.org/obo/GAZ_00041536 -->

    <owl:NamedIndividual rdf:about="http://purl.obolibrary.org/obo/GAZ_00041536">
        <obo:RO_0001025 rdf:resource="http://purl.obolibrary.org/obo/GAZ_00000007"/>
        <obo:RO_0001025 rdf:resource="http://purl.obolibrary.org/obo/GAZ_00136138"/>
        <obo:IAO_0000115>An endorheic soda lake located south of the Serengeti National Park and immediately southwest of the Ngorongoro Crater in the Crater Highlands area of Tanzania.</obo:IAO_0000115>
        <oboInOwl:hasOBONamespace>GAZ</oboInOwl:hasOBONamespace>
        <oboInOwl:id>GAZ:00041536</oboInOwl:id>
        <rdfs:label>Lake Eyasi</rdfs:label>
    </owl:NamedIndividual>
    


    <!-- http://purl.obolibrary.org/obo/GAZ_00041537 -->

    <owl:NamedIndividual rdf:about="http://purl.obolibrary.org/obo/GAZ_00041537">
        <obo:RO_0001025 rdf:resource="http://purl.obolibrary.org/obo/GAZ_00000007"/>
        <obo:IAO_0000115>A holopolymictic freshwater lake in Kenya, lying north west of Nairobi, outside the town of Naivasha. It is part of the Great Rift Valley. A Ramsar Site.</obo:IAO_0000115>
        <oboInOwl:hasOBONamespace>GAZ</oboInOwl:hasOBONamespace>
        <oboInOwl:id>GAZ:00041537</oboInOwl:id>
        <rdfs:label>Lake Naivasha</rdfs:label>
    </owl:NamedIndividual>
    


    <!-- http://purl.obolibrary.org/obo/GAZ_00041538 -->

    <owl:NamedIndividual rdf:about="http://purl.obolibrary.org/obo/GAZ_00041538">
        <obo:RO_0001025 rdf:resource="http://purl.obolibrary.org/obo/GAZ_00000007"/>
        <obo:RO_0001025 rdf:resource="http://purl.obolibrary.org/obo/GAZ_00000786"/>
        <obo:IAO_0000115>A monomictic alkaline endorheic lake.</obo:IAO_0000115>
        <oboInOwl:hasOBONamespace>GAZ</oboInOwl:hasOBONamespace>
        <oboInOwl:id>GAZ:00041538</oboInOwl:id>
        <rdfs:label>Lake Turkana</rdfs:label>
    </owl:NamedIndividual>
    


    <!-- http://purl.obolibrary.org/obo/GAZ_00041539 -->

    <owl:NamedIndividual rdf:about="http://purl.obolibrary.org/obo/GAZ_00041539">
        <obo:RO_0001025 rdf:resource="http://purl.obolibrary.org/obo/GAZ_00000007"/>
        <obo:IAO_0000115>A freshwater lake fed by several rivers. It has no obvious outlet; the waters seep into lava. A Ramsar Site.</obo:IAO_0000115>
        <oboInOwl:hasOBONamespace>GAZ</oboInOwl:hasOBONamespace>
        <oboInOwl:id>GAZ:00041539</oboInOwl:id>
        <rdfs:label>Lake Baringo</rdfs:label>
    </owl:NamedIndividual>
    


    <!-- http://purl.obolibrary.org/obo/GAZ_00041540 -->

    <owl:NamedIndividual rdf:about="http://purl.obolibrary.org/obo/GAZ_00041540">
        <obo:RO_0001025 rdf:resource="http://purl.obolibrary.org/obo/GAZ_00000007"/>
        <obo:RO_0001025 rdf:resource="http://purl.obolibrary.org/obo/GAZ_00236097"/>
        <obo:IAO_0000115>A saline, alkaline lake that lies at the northern end of the arid Suguta Valley in the northern Kenya Rift. It is separated from Lake Turkana by the Barrier volcanic complex, a group of young volcanoes that last erupted during the late 19th Century or early 20th Century. Saline hot springs discharge on the northern shoreline of Lake Logipi and at Cathedral Rocks near its southern limit, and help to maintain water at times of extreme aridity. During the rainy season, the lake is also recharged from the Suguta River which flows northward along the Suguta Valley, periodically forming a temporary lake (Lake Alablab) that unites with Logipi.</obo:IAO_0000115>
        <oboInOwl:hasOBONamespace>GAZ</oboInOwl:hasOBONamespace>
        <oboInOwl:id>GAZ:00041540</oboInOwl:id>
        <rdfs:label>Lake Logipi</rdfs:label>
    </owl:NamedIndividual>
    


    <!-- http://purl.obolibrary.org/obo/GAZ_00041541 -->

    <owl:NamedIndividual rdf:about="http://purl.obolibrary.org/obo/GAZ_00041541">
        <obo:RO_0001025 rdf:resource="http://purl.obolibrary.org/obo/GAZ_00041539"/>
        <obo:IAO_0000115>An Island in the center of Lake Baringo SW of Korosi volcano consists of young basaltic scoria cones that cap a trachytic shield volcano. The volcano is the smallest in the northern part of the Kenya rift valley. N-S-trending faults cut the complex, producing west-facing scarps. Smaller islands to the north and south are faulted basaltic lava flows; Parmalok Island to the SW is a breached trachytic tuff cone that fed a small lava flow. Hot springs, boiling mud pools, and fumaroles are present along the faults on the NE peninsula of the island.</obo:IAO_0000115>
        <oboInOwl:hasOBONamespace>GAZ</oboInOwl:hasOBONamespace>
        <oboInOwl:id>GAZ:00041541</oboInOwl:id>
        <rdfs:label>Ol Kokwe Island</rdfs:label>
    </owl:NamedIndividual>
    


    <!-- http://purl.obolibrary.org/obo/GAZ_00041542 -->

    <owl:NamedIndividual rdf:about="http://purl.obolibrary.org/obo/GAZ_00041542">
        <obo:RO_0001025 rdf:resource="http://purl.obolibrary.org/obo/GAZ_00041538"/>
        <obo:IAO_0000115>The northernmost and smallest of three volcanic islands in the Lake Turkana. North Island is the summit of Kenya&apos;s northernmost rift valley volcano and is primarily composed of trachyandesitic-to-trachytic phreatomagmatic deposits from overlapping eroded tuff cones or tuff rings. The center of the island consists of a young tuff ring about 1 km in diameter nested inside an older tuff ring. Two fresh unvegetated lava flows that reach the lake shore from the central tuff ring form lava deltas at the northern and western sides of the island; the northern delta is about 900 m wide.</obo:IAO_0000115>
        <oboInOwl:hasOBONamespace>GAZ</oboInOwl:hasOBONamespace>
        <oboInOwl:id>GAZ:00041542</oboInOwl:id>
        <rdfs:label>North Island</rdfs:label>
    </owl:NamedIndividual>
    


    <!-- http://purl.obolibrary.org/obo/GAZ_00041543 -->

    <owl:NamedIndividual rdf:about="http://purl.obolibrary.org/obo/GAZ_00041543">
        <obo:RO_0001025 rdf:resource="http://purl.obolibrary.org/obo/GAZ_00041538"/>
        <obo:IAO_0000115>An island that occupies the middle of Lake Turkana and is composed of more than a dozen craters and cones, three of which are filled by small lakes. The two largest lakes partially fill craters up to a km wide and about 80 m deep whose floors lie near sea level. The highest point on the dominantly basaltic island reaches 550 m, about 170 m above the lake surface. An E-W-trending chain of small explosion craters cuts the eastern side of the 3 km wide island. Several small islands to the SE represent partially submerged crater rims, and other cones and lava plugs lie beneath the lake surface near the island.</obo:IAO_0000115>
        <oboInOwl:hasOBONamespace>GAZ</oboInOwl:hasOBONamespace>
        <oboInOwl:id>GAZ:00041543</oboInOwl:id>
        <rdfs:label>Central Island</rdfs:label>
    </owl:NamedIndividual>
    


    <!-- http://purl.obolibrary.org/obo/GAZ_00041544 -->

    <owl:NamedIndividual rdf:about="http://purl.obolibrary.org/obo/GAZ_00041544">
        <obo:RO_0001025 rdf:resource="http://purl.obolibrary.org/obo/GAZ_00041538"/>
        <obo:IAO_0000115>An island that contains numerous tuff cones. Fresh-looking lava flows, erupted from a N-S fissure extending the 11 km length of the island, form much of the eastern shoreline. South Island rises 320 m above the lake to a height of 800 m and is part of a volcanic horst that extends 10 km to the north beneath the lake surface.</obo:IAO_0000115>
        <oboInOwl:hasOBONamespace>GAZ</oboInOwl:hasOBONamespace>
        <oboInOwl:id>GAZ:00041544</oboInOwl:id>
        <rdfs:label>South Island</rdfs:label>
    </owl:NamedIndividual>
    


    <!-- http://purl.obolibrary.org/obo/GAZ_00041545 -->

    <owl:NamedIndividual rdf:about="http://purl.obolibrary.org/obo/GAZ_00041545">
        <obo:RO_0001025 rdf:resource="http://purl.obolibrary.org/obo/GAZ_00041530"/>
        <obo:IAO_0000115>An island in Lake Mweru.</obo:IAO_0000115>
        <oboInOwl:hasOBONamespace>GAZ</oboInOwl:hasOBONamespace>
        <oboInOwl:id>GAZ:00041545</oboInOwl:id>
        <rdfs:label>Kilwa Island</rdfs:label>
    </owl:NamedIndividual>
    


    <!-- http://purl.obolibrary.org/obo/GAZ_00041546 -->

    <owl:NamedIndividual rdf:about="http://purl.obolibrary.org/obo/GAZ_00041546">
        <obo:RO_0001025 rdf:resource="http://purl.obolibrary.org/obo/GAZ_00041530"/>
        <oboInOwl:hasOBONamespace>GAZ</oboInOwl:hasOBONamespace>
        <oboInOwl:id>GAZ:00041546</oboInOwl:id>
        <rdfs:label>Isokwe Island</rdfs:label>
    </owl:NamedIndividual>
    


    <!-- http://purl.obolibrary.org/obo/GAZ_00041547 -->

    <owl:NamedIndividual rdf:about="http://purl.obolibrary.org/obo/GAZ_00041547">
        <obo:RO_0001025 rdf:resource="http://purl.obolibrary.org/obo/GAZ_00041534"/>
        <oboInOwl:hasOBONamespace>GAZ</oboInOwl:hasOBONamespace>
        <oboInOwl:id>GAZ:00041547</oboInOwl:id>
        <rdfs:label>Rukwanzi Island</rdfs:label>
    </owl:NamedIndividual>
    


    <!-- http://purl.obolibrary.org/obo/GAZ_00041548 -->

    <owl:NamedIndividual rdf:about="http://purl.obolibrary.org/obo/GAZ_00041548">
        <obo:RO_0001025 rdf:resource="http://purl.obolibrary.org/obo/GAZ_00041537"/>
        <obo:IAO_0000115>An island of Lake Naivasha.</obo:IAO_0000115>
        <oboInOwl:hasOBONamespace>GAZ</oboInOwl:hasOBONamespace>
        <oboInOwl:id>GAZ:00041548</oboInOwl:id>
        <rdfs:label>Crescent Island</rdfs:label>
    </owl:NamedIndividual>
    


    <!-- http://purl.obolibrary.org/obo/GAZ_00041549 -->

    <owl:NamedIndividual rdf:about="http://purl.obolibrary.org/obo/GAZ_00041549">
        <obo:RO_0001025 rdf:resource="http://purl.obolibrary.org/obo/GAZ_00053591"/>
        <obo:IAO_0000115>A polymictic soda lake. A Ramsar Site.</obo:IAO_0000115>
        <oboInOwl:hasOBONamespace>GAZ</oboInOwl:hasOBONamespace>
        <oboInOwl:id>GAZ:00041549</oboInOwl:id>
        <rdfs:label>Lake Nakuru</rdfs:label>
    </owl:NamedIndividual>
    


    <!-- http://purl.obolibrary.org/obo/GAZ_00041550 -->

    <owl:NamedIndividual rdf:about="http://purl.obolibrary.org/obo/GAZ_00041550">
        <obo:RO_0001025 rdf:resource="http://purl.obolibrary.org/obo/GAZ_00000007"/>
        <obo:RO_0001025 rdf:resource="http://purl.obolibrary.org/obo/GAZ_00000780"/>
        <obo:RO_0001025 rdf:resource="http://purl.obolibrary.org/obo/GAZ_00123543"/>
        <obo:IAO_0000115>A lake that is the source of the Blue Nile and is the largest lake in Ethiopia. Located in the north-western Ethiopian highlands. Lake Tana is fed by the Little Abay, Reb and Gumara Rivers.</obo:IAO_0000115>
        <oboInOwl:hasOBONamespace>GAZ</oboInOwl:hasOBONamespace>
        <oboInOwl:id>GAZ:00041550</oboInOwl:id>
        <rdfs:label>Lake Tana</rdfs:label>
    </owl:NamedIndividual>
    


    <!-- http://purl.obolibrary.org/obo/GAZ_00041551 -->

    <owl:NamedIndividual rdf:about="http://purl.obolibrary.org/obo/GAZ_00041551">
        <obo:RO_0001025 rdf:resource="http://purl.obolibrary.org/obo/GAZ_00041550"/>
        <obo:IAO_0000115>An island in Lake Tana in Ethiopia.</obo:IAO_0000115>
        <oboInOwl:hasOBONamespace>GAZ</oboInOwl:hasOBONamespace>
        <oboInOwl:id>GAZ:00041551</oboInOwl:id>
        <rdfs:label>Tana Qirqos Island</rdfs:label>
    </owl:NamedIndividual>
    


    <!-- http://purl.obolibrary.org/obo/GAZ_00041552 -->

    <owl:NamedIndividual rdf:about="http://purl.obolibrary.org/obo/GAZ_00041552">
        <obo:RO_0001025 rdf:resource="http://purl.obolibrary.org/obo/GAZ_00041550"/>
        <obo:IAO_0000115>An island of Lake Tana.</obo:IAO_0000115>
        <oboInOwl:hasOBONamespace>GAZ</oboInOwl:hasOBONamespace>
        <oboInOwl:id>GAZ:00041552</oboInOwl:id>
        <rdfs:label>Meshralia Island</rdfs:label>
    </owl:NamedIndividual>
    


    <!-- http://purl.obolibrary.org/obo/GAZ_00041553 -->

    <owl:NamedIndividual rdf:about="http://purl.obolibrary.org/obo/GAZ_00041553">
        <obo:RO_0001025 rdf:resource="http://purl.obolibrary.org/obo/GAZ_00041550"/>
        <obo:IAO_0000115>An island of Lake Tana.</obo:IAO_0000115>
        <oboInOwl:hasOBONamespace>GAZ</oboInOwl:hasOBONamespace>
        <oboInOwl:id>GAZ:00041553</oboInOwl:id>
        <rdfs:label>Daga Island</rdfs:label>
    </owl:NamedIndividual>
    


    <!-- http://purl.obolibrary.org/obo/GAZ_00041554 -->

    <owl:NamedIndividual rdf:about="http://purl.obolibrary.org/obo/GAZ_00041554">
        <obo:RO_0001025 rdf:resource="http://purl.obolibrary.org/obo/GAZ_00041550"/>
        <obo:RO_0001025 rdf:resource="http://purl.obolibrary.org/obo/GAZ_00123475"/>
        <obo:IAO_0000115>The biggest island (approximately 16 km2) on Lake Tana in Ethiopia. It is administratively included in the Achefer woreda of the Mirab Gojjam Zone.</obo:IAO_0000115>
        <oboInOwl:hasOBONamespace>GAZ</oboInOwl:hasOBONamespace>
        <oboInOwl:id>GAZ:00041554</oboInOwl:id>
        <rdfs:label>Dek Island</rdfs:label>
    </owl:NamedIndividual>
    


    <!-- http://purl.obolibrary.org/obo/GAZ_00041555 -->

    <owl:NamedIndividual rdf:about="http://purl.obolibrary.org/obo/GAZ_00041555">
        <obo:RO_0001025 rdf:resource="http://purl.obolibrary.org/obo/GAZ_00000007"/>
        <obo:RO_0001025 rdf:resource="http://purl.obolibrary.org/obo/GAZ_00000567"/>
        <obo:IAO_0000115>A freshwater Rift Valley lake of Ethiopia. It is located about 60 miles south of Addis Ababa, on the border between the regions (or kililoch) of Oromia and of the Southern Nations, Nationalities, and Peoples. The lake is fed primarily by two rivers, the Meki and the Katar, but does not always have an outflow, although in some years it drains into Lake Abijatta.</obo:IAO_0000115>
        <oboInOwl:hasOBONamespace>GAZ</oboInOwl:hasOBONamespace>
        <oboInOwl:id>GAZ:00041555</oboInOwl:id>
        <rdfs:label>Lake Zway</rdfs:label>
    </owl:NamedIndividual>
    


    <!-- http://purl.obolibrary.org/obo/GAZ_00041556 -->

    <owl:NamedIndividual rdf:about="http://purl.obolibrary.org/obo/GAZ_00041556">
        <obo:RO_0001025 rdf:resource="http://purl.obolibrary.org/obo/GAZ_00000007"/>
        <obo:RO_0001025 rdf:resource="http://purl.obolibrary.org/obo/GAZ_00123871"/>
        <obo:IAO_0000115>A polymictic freshwater lake in Ethiopia, located in the Rift Valley south of Addis Ababa. Thought to have a subterranean outlet.</obo:IAO_0000115>
        <oboInOwl:hasOBONamespace>GAZ</oboInOwl:hasOBONamespace>
        <oboInOwl:id>GAZ:00041556</oboInOwl:id>
        <rdfs:label>Lake Awasa</rdfs:label>
    </owl:NamedIndividual>
    


    <!-- http://purl.obolibrary.org/obo/GAZ_00041557 -->

    <owl:NamedIndividual rdf:about="http://purl.obolibrary.org/obo/GAZ_00041557">
        <obo:RO_0001025 rdf:resource="http://purl.obolibrary.org/obo/GAZ_00000007"/>
        <obo:RO_0001025 rdf:resource="http://purl.obolibrary.org/obo/GAZ_00000784"/>
        <obo:IAO_0000115>A lake in Ethiopia.</obo:IAO_0000115>
        <oboInOwl:hasOBONamespace>GAZ</oboInOwl:hasOBONamespace>
        <oboInOwl:id>GAZ:00041557</oboInOwl:id>
        <rdfs:label>Lake Koka</rdfs:label>
    </owl:NamedIndividual>
    


    <!-- http://purl.obolibrary.org/obo/GAZ_00041559 -->

    <owl:NamedIndividual rdf:about="http://purl.obolibrary.org/obo/GAZ_00041559">
        <obo:RO_0001025 rdf:resource="http://purl.obolibrary.org/obo/GAZ_00000007"/>
        <obo:RO_0001025 rdf:resource="http://purl.obolibrary.org/obo/GAZ_00053666"/>
        <obo:RO_0001025 rdf:resource="http://purl.obolibrary.org/obo/GAZ_00123873"/>
        <obo:IAO_0000115>An endorheic alkaline lake in Ethiopia south of Addis Ababa, in the Abijatta-Shalla National Park.</obo:IAO_0000115>
        <oboInOwl:hasOBONamespace>GAZ</oboInOwl:hasOBONamespace>
        <oboInOwl:id>GAZ:00041559</oboInOwl:id>
        <rdfs:label>Lake Abijatta</rdfs:label>
    </owl:NamedIndividual>
    


    <!-- http://purl.obolibrary.org/obo/GAZ_00041560 -->

    <owl:NamedIndividual rdf:about="http://purl.obolibrary.org/obo/GAZ_00041560">
        <obo:RO_0001025 rdf:resource="http://purl.obolibrary.org/obo/GAZ_00000007"/>
        <obo:RO_0001025 rdf:resource="http://purl.obolibrary.org/obo/GAZ_00053676"/>
        <obo:RO_0001025 rdf:resource="http://purl.obolibrary.org/obo/GAZ_00123681"/>
        <obo:RO_0001025 rdf:resource="http://purl.obolibrary.org/obo/GAZ_00123779"/>
        <obo:IAO_0000115>A lake in the Southern Nations, Nationalities, and Peoples Region of Ethiopia. Located in the Great Rift Valley, east of the Guge Mountains. It is fed on its northern shore by the Bilate River, which rises on the southern slopes of Mount Gurage.</obo:IAO_0000115>
        <oboInOwl:hasOBONamespace>GAZ</oboInOwl:hasOBONamespace>
        <oboInOwl:id>GAZ:00041560</oboInOwl:id>
        <rdfs:label>Lake Abaya</rdfs:label>
    </owl:NamedIndividual>
    


    <!-- http://purl.obolibrary.org/obo/GAZ_00041561 -->

    <owl:NamedIndividual rdf:about="http://purl.obolibrary.org/obo/GAZ_00041561">
        <obo:RO_0001025 rdf:resource="http://purl.obolibrary.org/obo/GAZ_00041560"/>
        <oboInOwl:hasOBONamespace>GAZ</oboInOwl:hasOBONamespace>
        <oboInOwl:id>GAZ:00041561</oboInOwl:id>
        <rdfs:label>Aruro Island</rdfs:label>
    </owl:NamedIndividual>
    


    <!-- http://purl.obolibrary.org/obo/GAZ_00041562 -->

    <owl:NamedIndividual rdf:about="http://purl.obolibrary.org/obo/GAZ_00041562">
        <obo:RO_0001025 rdf:resource="http://purl.obolibrary.org/obo/GAZ_00041555"/>
        <obo:IAO_0000115>An island of Lake Zway.</obo:IAO_0000115>
        <oboInOwl:hasOBONamespace>GAZ</oboInOwl:hasOBONamespace>
        <oboInOwl:id>GAZ:00041562</oboInOwl:id>
        <rdfs:label>Galila Island</rdfs:label>
    </owl:NamedIndividual>
    


    <!-- http://purl.obolibrary.org/obo/GAZ_00041563 -->

    <owl:NamedIndividual rdf:about="http://purl.obolibrary.org/obo/GAZ_00041563">
        <obo:RO_0001025 rdf:resource="http://purl.obolibrary.org/obo/GAZ_00015452"/>
        <obo:IAO_0000115>An island in Lake Victoria.</obo:IAO_0000115>
        <oboInOwl:hasOBONamespace>GAZ</oboInOwl:hasOBONamespace>
        <oboInOwl:id>GAZ:00041563</oboInOwl:id>
        <rdfs:label>Lolui Island</rdfs:label>
    </owl:NamedIndividual>
    


    <!-- http://purl.obolibrary.org/obo/GAZ_00041564 -->

    <owl:NamedIndividual rdf:about="http://purl.obolibrary.org/obo/GAZ_00041564">
        <obo:RO_0001025 rdf:resource="http://purl.obolibrary.org/obo/GAZ_00041555"/>
        <obo:IAO_0000115>An island of Lake Zway.</obo:IAO_0000115>
        <oboInOwl:hasOBONamespace>GAZ</oboInOwl:hasOBONamespace>
        <oboInOwl:id>GAZ:00041564</oboInOwl:id>
        <rdfs:label>Tullu Gudo Island</rdfs:label>
    </owl:NamedIndividual>
    


    <!-- http://purl.obolibrary.org/obo/GAZ_00041565 -->

    <owl:NamedIndividual rdf:about="http://purl.obolibrary.org/obo/GAZ_00041565">
        <obo:RO_0001025 rdf:resource="http://purl.obolibrary.org/obo/GAZ_00041555"/>
        <obo:IAO_0000115>An island of Lake Zway.</obo:IAO_0000115>
        <oboInOwl:hasOBONamespace>GAZ</oboInOwl:hasOBONamespace>
        <oboInOwl:id>GAZ:00041565</oboInOwl:id>
        <rdfs:label>Bird Island</rdfs:label>
    </owl:NamedIndividual>
    


    <!-- http://purl.obolibrary.org/obo/GAZ_00041566 -->

    <owl:NamedIndividual rdf:about="http://purl.obolibrary.org/obo/GAZ_00041566">
        <obo:RO_0001025 rdf:resource="http://purl.obolibrary.org/obo/GAZ_00041555"/>
        <obo:IAO_0000115>An island of Lake Zway.</obo:IAO_0000115>
        <oboInOwl:hasOBONamespace>GAZ</oboInOwl:hasOBONamespace>
        <oboInOwl:id>GAZ:00041566</oboInOwl:id>
        <rdfs:label>Debre Sina Island</rdfs:label>
    </owl:NamedIndividual>
    


    <!-- http://purl.obolibrary.org/obo/GAZ_00041571 -->

    <owl:NamedIndividual rdf:about="http://purl.obolibrary.org/obo/GAZ_00041571">
        <obo:RO_0001025 rdf:resource="http://purl.obolibrary.org/obo/GAZ_00015452"/>
        <obo:IAO_0000115>An island in Lake Victoria.</obo:IAO_0000115>
        <oboInOwl:hasOBONamespace>GAZ</oboInOwl:hasOBONamespace>
        <oboInOwl:id>GAZ:00041571</oboInOwl:id>
        <rdfs:label>Iroba Island</rdfs:label>
    </owl:NamedIndividual>
    


    <!-- http://purl.obolibrary.org/obo/GAZ_00041572 -->

    <owl:NamedIndividual rdf:about="http://purl.obolibrary.org/obo/GAZ_00041572">
        <obo:RO_0001025 rdf:resource="http://purl.obolibrary.org/obo/GAZ_00052895"/>
        <obo:IAO_0000115>An island that lies in the eastern part of Lake Victoria, at the mouth of the Winam Gulf. Part of Kenya, it lies west of Rusinga Island.</obo:IAO_0000115>
        <oboInOwl:hasOBONamespace>GAZ</oboInOwl:hasOBONamespace>
        <oboInOwl:id>GAZ:00041572</oboInOwl:id>
        <rdfs:label>Mfangano Island</rdfs:label>
    </owl:NamedIndividual>
    


    <!-- http://purl.obolibrary.org/obo/GAZ_00041573 -->

    <owl:NamedIndividual rdf:about="http://purl.obolibrary.org/obo/GAZ_00041573">
        <obo:RO_0001025 rdf:resource="http://purl.obolibrary.org/obo/GAZ_00015452"/>
        <obo:IAO_0000115>An island in Lake Victoria.</obo:IAO_0000115>
        <oboInOwl:hasOBONamespace>GAZ</oboInOwl:hasOBONamespace>
        <oboInOwl:id>GAZ:00041573</oboInOwl:id>
        <rdfs:label>Ukara Island</rdfs:label>
    </owl:NamedIndividual>
    


    <!-- http://purl.obolibrary.org/obo/GAZ_00041574 -->

    <owl:NamedIndividual rdf:about="http://purl.obolibrary.org/obo/GAZ_00041574">
        <obo:RO_0001025 rdf:resource="http://purl.obolibrary.org/obo/GAZ_00015452"/>
        <obo:IAO_0000115>An island in Lake Victoria.</obo:IAO_0000115>
        <oboInOwl:hasOBONamespace>GAZ</oboInOwl:hasOBONamespace>
        <oboInOwl:id>GAZ:00041574</oboInOwl:id>
        <rdfs:label>Kome Island [South]</rdfs:label>
    </owl:NamedIndividual>
    


    <!-- http://purl.obolibrary.org/obo/GAZ_00041575 -->

    <owl:NamedIndividual rdf:about="http://purl.obolibrary.org/obo/GAZ_00041575">
        <obo:RO_0001025 rdf:resource="http://purl.obolibrary.org/obo/GAZ_00015452"/>
        <obo:IAO_0000115>A small island in Lake Victoria, Tanzania.</obo:IAO_0000115>
        <oboInOwl:hasOBONamespace>GAZ</oboInOwl:hasOBONamespace>
        <oboInOwl:id>GAZ:00041575</oboInOwl:id>
        <rdfs:label>Nabuyongo Island</rdfs:label>
    </owl:NamedIndividual>
    


    <!-- http://purl.obolibrary.org/obo/GAZ_00041576 -->

    <owl:NamedIndividual rdf:about="http://purl.obolibrary.org/obo/GAZ_00041576">
        <obo:RO_0001025 rdf:resource="http://purl.obolibrary.org/obo/GAZ_00015452"/>
        <obo:IAO_0000115>An island in Lake Victoria.</obo:IAO_0000115>
        <oboInOwl:hasOBONamespace>GAZ</oboInOwl:hasOBONamespace>
        <oboInOwl:id>GAZ:00041576</oboInOwl:id>
        <rdfs:label>Bumbire Island</rdfs:label>
    </owl:NamedIndividual>
    


    <!-- http://purl.obolibrary.org/obo/GAZ_00041577 -->

    <owl:NamedIndividual rdf:about="http://purl.obolibrary.org/obo/GAZ_00041577">
        <obo:RO_0001025 rdf:resource="http://purl.obolibrary.org/obo/GAZ_00015452"/>
        <obo:IAO_0000115>An island in Lake Victoria.</obo:IAO_0000115>
        <oboInOwl:hasOBONamespace>GAZ</oboInOwl:hasOBONamespace>
        <oboInOwl:id>GAZ:00041577</oboInOwl:id>
        <rdfs:label>Kome Island [North]</rdfs:label>
    </owl:NamedIndividual>
    


    <!-- http://purl.obolibrary.org/obo/GAZ_00041578 -->

    <owl:NamedIndividual rdf:about="http://purl.obolibrary.org/obo/GAZ_00041578">
        <obo:RO_0001025 rdf:resource="http://purl.obolibrary.org/obo/GAZ_00015452"/>
        <obo:IAO_0000115>An island in Lake Victoria.</obo:IAO_0000115>
        <oboInOwl:hasOBONamespace>GAZ</oboInOwl:hasOBONamespace>
        <oboInOwl:id>GAZ:00041578</oboInOwl:id>
        <rdfs:label>Ikuza Island</rdfs:label>
    </owl:NamedIndividual>
    


    <!-- http://purl.obolibrary.org/obo/GAZ_00041579 -->

    <owl:NamedIndividual rdf:about="http://purl.obolibrary.org/obo/GAZ_00041579">
        <obo:RO_0001025 rdf:resource="http://purl.obolibrary.org/obo/GAZ_00015452"/>
        <obo:IAO_0000115>An island that lies in the eastern part of Lake Victoria at the mouth of the Winam Gulf. Part of Kenya, it is linked to Mbita Point on the mainland by a causeway.</obo:IAO_0000115>
        <oboInOwl:hasOBONamespace>GAZ</oboInOwl:hasOBONamespace>
        <oboInOwl:id>GAZ:00041579</oboInOwl:id>
        <rdfs:label>Rusinga Island</rdfs:label>
    </owl:NamedIndividual>
    


    <!-- http://purl.obolibrary.org/obo/GAZ_00041580 -->

    <owl:NamedIndividual rdf:about="http://purl.obolibrary.org/obo/GAZ_00041580">
        <obo:RO_0001025 rdf:resource="http://purl.obolibrary.org/obo/GAZ_00052895"/>
        <obo:IAO_0000115>A small island (4.2 km2) in Winam Gulf of Lake Victoria in Kenya.</obo:IAO_0000115>
        <oboInOwl:hasOBONamespace>GAZ</oboInOwl:hasOBONamespace>
        <oboInOwl:id>GAZ:00041580</oboInOwl:id>
        <rdfs:label>Ndere Island</rdfs:label>
    </owl:NamedIndividual>
    


    <!-- http://purl.obolibrary.org/obo/GAZ_00041581 -->

    <owl:NamedIndividual rdf:about="http://purl.obolibrary.org/obo/GAZ_00041581">
        <obo:RO_0001025 rdf:resource="http://purl.obolibrary.org/obo/GAZ_00015452"/>
        <obo:IAO_0000115>An island in Lake Victoria.</obo:IAO_0000115>
        <oboInOwl:hasOBONamespace>GAZ</oboInOwl:hasOBONamespace>
        <oboInOwl:id>GAZ:00041581</oboInOwl:id>
        <rdfs:label>Bukasa Island</rdfs:label>
    </owl:NamedIndividual>
    


    <!-- http://purl.obolibrary.org/obo/GAZ_00041582 -->

    <owl:NamedIndividual rdf:about="http://purl.obolibrary.org/obo/GAZ_00041582">
        <obo:RO_0001025 rdf:resource="http://purl.obolibrary.org/obo/GAZ_00015452"/>
        <obo:IAO_0000115>A small island in northern Lake Victoria. It is about 10 km south of Kampala, Uganda.</obo:IAO_0000115>
        <oboInOwl:hasOBONamespace>GAZ</oboInOwl:hasOBONamespace>
        <oboInOwl:id>GAZ:00041582</oboInOwl:id>
        <rdfs:label>Bulingugwe Island</rdfs:label>
    </owl:NamedIndividual>
    


    <!-- http://purl.obolibrary.org/obo/GAZ_00044906 -->

    <owl:NamedIndividual rdf:about="http://purl.obolibrary.org/obo/GAZ_00044906">
        <obo:RO_0001025 rdf:resource="http://purl.obolibrary.org/obo/GAZ_00000007"/>
        <obo:IAO_0000115>A fertile valley in east Lebanon. Located about 30 km east of Beirut. The valley is situated between the Mount Lebanon to the west and the Anti-Lebanon mountain ranges to the east. It forms the northeasternmost extension of the Great Rift Valley, which stretches from Syria through the Red Sea into Africa. Beqaa Valley is about 120 km in length and has an average width of about 16 km.</obo:IAO_0000115>
        <oboInOwl:hasOBONamespace>GAZ</oboInOwl:hasOBONamespace>
        <oboInOwl:id>GAZ:00044906</oboInOwl:id>
        <rdfs:label>Beqaa Valley</rdfs:label>
    </owl:NamedIndividual>
    


    <!-- http://purl.obolibrary.org/obo/GAZ_00044911 -->

    <owl:NamedIndividual rdf:about="http://purl.obolibrary.org/obo/GAZ_00044911">
        <obo:RO_0001025 rdf:resource="http://purl.obolibrary.org/obo/GAZ_00248126"/>
        <obo:IAO_0000115>An endorheic saline lake in Southern Ethiopia on the boundary between the Oromia and the Southern Nations, Nationalities and Peoples&apos; Regions. When the lake is filled, it stretches into northern Kenya. Lying at the center of the Stephanie Wildlife Reserve, the lake measures some 40 miles by 15 miles. This lake is the southernmost and lowest (1,880 feet) of a series of lakes which lie in the north-easterly continuation of the Great Rift Valley; its watershed is separated from the watershed of Lake Turkana by the Humu Range and the hills south of it. The Kumbi Range rises on its eastern side. Chew Bahir is fed from the north by the Weito River, and its tributary the Galana Sagan. The Galana Sagan receives the overflow of Lake Chamo in some years, but no permanent connection exists.</obo:IAO_0000115>
        <oboInOwl:hasOBONamespace>GAZ</oboInOwl:hasOBONamespace>
        <oboInOwl:id>GAZ:00044911</oboInOwl:id>
        <rdfs:label>Lake Bahir</rdfs:label>
    </owl:NamedIndividual>
    


    <!-- http://purl.obolibrary.org/obo/GAZ_00044914 -->

    <owl:NamedIndividual rdf:about="http://purl.obolibrary.org/obo/GAZ_00044914">
        <obo:RO_0001025 rdf:resource="http://purl.obolibrary.org/obo/GAZ_00007520"/>
        <obo:IAO_0000115>A freshwater monomictic lake, being approximately 53 km in circumference, about 21 km long, and 13 km wide. The lake has a total area of 166 km2, and a maximum depth of approximately 43 m. It is situated deep in the Jordan Great Rift Valley, the valley caused by the separation of the African and Arabian Plates and is fed partly by underground springs although its main source is the Jordan River which flows through it from north to south. Consequently the area is subject to earthquakes and, in the past, volcanic activity. This is evidenced by the abundant basalt and other igneous rocks that define the geology of the Galilee region.</obo:IAO_0000115>
        <oboInOwl:hasOBONamespace>GAZ</oboInOwl:hasOBONamespace>
        <oboInOwl:id>GAZ:00044914</oboInOwl:id>
        <rdfs:label>Sea of Galilee</rdfs:label>
    </owl:NamedIndividual>
    


    <!-- http://purl.obolibrary.org/obo/GAZ_00044915 -->

    <owl:NamedIndividual rdf:about="http://purl.obolibrary.org/obo/GAZ_00044915">
        <obo:RO_0001025 rdf:resource="http://purl.obolibrary.org/obo/GAZ_00000007"/>
        <obo:IAO_0000115>A 375 km long strike-slip fault zone some 5 km wide in the north and 23 km wide in the south that forms part of the broader Great Rift Valley. Located in modern-day Israel, Jordan, the West Bank and the Golan Heights, this geographic region includes the Jordan River, Hula Valley, Lake Tiberias and the Dead Sea, features created by the physiographic and geologic process underway.</obo:IAO_0000115>
        <oboInOwl:hasOBONamespace>GAZ</oboInOwl:hasOBONamespace>
        <oboInOwl:id>GAZ:00044915</oboInOwl:id>
        <rdfs:label>Jordan Rift Valley</rdfs:label>
    </owl:NamedIndividual>
    


    <!-- http://purl.obolibrary.org/obo/GAZ_00044916 -->

    <owl:NamedIndividual rdf:about="http://purl.obolibrary.org/obo/GAZ_00044916">
        <obo:RO_0001025 rdf:resource="http://purl.obolibrary.org/obo/GAZ_00000007"/>
        <obo:RO_0001025 rdf:resource="http://purl.obolibrary.org/obo/GAZ_00044915"/>
        <obo:IAO_0000115>A section of the Great Rift Valley lying between the Dead Sea to the north and the Gulf of Aqaba or the Gulf of Eilat to the south. It forms part of the border between Israel to the west and Jordan to the east.</obo:IAO_0000115>
        <oboInOwl:hasOBONamespace>GAZ</oboInOwl:hasOBONamespace>
        <oboInOwl:id>GAZ:00044916</oboInOwl:id>
        <rdfs:label>Wadi Arabah</rdfs:label>
    </owl:NamedIndividual>
    


    <!-- http://purl.obolibrary.org/obo/GAZ_00049007 -->

    <owl:NamedIndividual rdf:about="http://purl.obolibrary.org/obo/GAZ_00049007">
        <obo:RO_0001025 rdf:resource="http://purl.obolibrary.org/obo/GAZ_00007862"/>
        <obo:IAO_0000115>The narrow sea passages, about 13 km wide, between the Sinai and Arabian peninsulas which separates the Gulf of Aqaba from the Red Sea.</obo:IAO_0000115>
        <oboInOwl:hasOBONamespace>GAZ</oboInOwl:hasOBONamespace>
        <oboInOwl:id>GAZ:00049007</oboInOwl:id>
        <rdfs:label>Straits of Tiran</rdfs:label>
    </owl:NamedIndividual>
    


    <!-- http://purl.obolibrary.org/obo/GAZ_00049008 -->

    <owl:NamedIndividual rdf:about="http://purl.obolibrary.org/obo/GAZ_00049008">
        <obo:RO_0001025 rdf:resource="http://purl.obolibrary.org/obo/GAZ_00049007"/>
        <obo:IAO_0000115>A Saudi Arabian island in the Straits of Tiran east of Tiran Island.</obo:IAO_0000115>
        <oboInOwl:hasOBONamespace>GAZ</oboInOwl:hasOBONamespace>
        <oboInOwl:id>GAZ:00049008</oboInOwl:id>
        <rdfs:label>Sanafir Island</rdfs:label>
    </owl:NamedIndividual>
    


    <!-- http://purl.obolibrary.org/obo/GAZ_00049009 -->

    <owl:NamedIndividual rdf:about="http://purl.obolibrary.org/obo/GAZ_00049009">
        <obo:RO_0001025 rdf:resource="http://purl.obolibrary.org/obo/GAZ_00049007"/>
        <obo:IAO_0000115>An island belonging to Saudi Arabia at the entrance of the Straits of Tiran, which separates the Red Sea and the Gulf of Aqaba.</obo:IAO_0000115>
        <oboInOwl:hasOBONamespace>GAZ</oboInOwl:hasOBONamespace>
        <oboInOwl:id>GAZ:00049009</oboInOwl:id>
        <rdfs:label>Tiran Island</rdfs:label>
    </owl:NamedIndividual>
    


    <!-- http://purl.obolibrary.org/obo/GAZ_00051205 -->

    <owl:NamedIndividual rdf:about="http://purl.obolibrary.org/obo/GAZ_00051205">
        <obo:RO_0001025 rdf:resource="http://purl.obolibrary.org/obo/GAZ_00000007"/>
        <obo:IAO_0000115>A geological depression in the Horn of Africa, where it overlaps Eritrea, the Afar Region of Ethiopia, and Djibouti. Only the Awash River flows into the depression, where it ends in a chain of lakes that increase in salinity.</obo:IAO_0000115>
        <oboInOwl:hasOBONamespace>GAZ</oboInOwl:hasOBONamespace>
        <oboInOwl:id>GAZ:00051205</oboInOwl:id>
        <rdfs:label>Afar Depression</rdfs:label>
    </owl:NamedIndividual>
    


    <!-- http://purl.obolibrary.org/obo/GAZ_00052521 -->

    <owl:NamedIndividual rdf:about="http://purl.obolibrary.org/obo/GAZ_00052521">
        <rdf:type rdf:resource="http://purl.obolibrary.org/obo/ENVO_00000856"/>
        <obo:RO_0001025 rdf:resource="http://purl.obolibrary.org/obo/GAZ_00052524"/>
        <obo:IAO_0000115>A populated place. A town in east-central Ethiopia. Located in the Misraq Hararghe Zone of the Oromia Region. One of the 180 woredas in the Oromia Region of Ethiopia. It is named after the woreda capital, Haro Maya.</obo:IAO_0000115>
        <oboInOwl:hasOBONamespace>GAZ</oboInOwl:hasOBONamespace>
        <oboInOwl:id>GAZ:00052521</oboInOwl:id>
        <rdfs:label>Alemaya</rdfs:label>
    </owl:NamedIndividual>
    


    <!-- http://purl.obolibrary.org/obo/GAZ_00052522 -->

    <owl:NamedIndividual rdf:about="http://purl.obolibrary.org/obo/GAZ_00052522">
        <obo:RO_0001025 rdf:resource="http://purl.obolibrary.org/obo/GAZ_00031125"/>
        <obo:IAO_0000115>One of the 180 woredas in the Oromia Region of Ethiopia. Part of the Mirab Shewa Zone, Ambo is bordered on the southwest by Tikur, on the west by Cheliya, on the north by Ginde Beret, on the northeast by Jeldu, on the east by Dendi, and on the southeast by Wonchi.</obo:IAO_0000115>
        <oboInOwl:hasOBONamespace>GAZ</oboInOwl:hasOBONamespace>
        <oboInOwl:id>GAZ:00052522</oboInOwl:id>
        <rdfs:label>Ambo Woreda</rdfs:label>
    </owl:NamedIndividual>
    


    <!-- http://purl.obolibrary.org/obo/GAZ_00052523 -->

    <owl:NamedIndividual rdf:about="http://purl.obolibrary.org/obo/GAZ_00052523">
        <obo:RO_0001025 rdf:resource="http://purl.obolibrary.org/obo/GAZ_00052522"/>
        <obo:IAO_0000115>A spa town in central Ethiopia. Located in the Mirab Shewa Zone of the Oromia Region, west of Addis Ababa.</obo:IAO_0000115>
        <oboInOwl:hasOBONamespace>GAZ</oboInOwl:hasOBONamespace>
        <oboInOwl:id>GAZ:00052523</oboInOwl:id>
        <rdfs:label>Ambo</rdfs:label>
    </owl:NamedIndividual>
    


    <!-- http://purl.obolibrary.org/obo/GAZ_00052524 -->

    <owl:NamedIndividual rdf:about="http://purl.obolibrary.org/obo/GAZ_00052524">
        <obo:RO_0001025 rdf:resource="http://purl.obolibrary.org/obo/GAZ_00031116"/>
        <obo:IAO_0000115>One of the 180 woredas in the Oromia Region of Ethiopia. Part of the Misraq (East) Hararghe Zone, Haro Maya is bordered on the south by Kurfa Chele, on the west by Kersa, on the north by Dire Dawa, on the east by Kombolcha, and on the southeast by the Harari Region. Towns include Alemaya and Bati.</obo:IAO_0000115>
        <oboInOwl:hasOBONamespace>GAZ</oboInOwl:hasOBONamespace>
        <oboInOwl:id>GAZ:00052524</oboInOwl:id>
        <rdfs:label>Haro Maya Woreda</rdfs:label>
    </owl:NamedIndividual>
    


    <!-- http://purl.obolibrary.org/obo/GAZ_00052529 -->

    <owl:NamedIndividual rdf:about="http://purl.obolibrary.org/obo/GAZ_00052529">
        <obo:RO_0001025 rdf:resource="http://purl.obolibrary.org/obo/GAZ_00031114"/>
        <obo:IAO_0000115>One of the 180 woredas in the Oromia Region of Ethiopia; it is named after the woreda capital, Adaba. Part of the Bale Zone.</obo:IAO_0000115>
        <oboInOwl:hasOBONamespace>GAZ</oboInOwl:hasOBONamespace>
        <oboInOwl:id>GAZ:00052529</oboInOwl:id>
        <rdfs:label>Sinanana Dinsho Woreda</rdfs:label>
    </owl:NamedIndividual>
    


    <!-- http://purl.obolibrary.org/obo/GAZ_00052530 -->

    <owl:NamedIndividual rdf:about="http://purl.obolibrary.org/obo/GAZ_00052530">
        <rdf:type rdf:resource="http://purl.obolibrary.org/obo/ENVO_00000856"/>
        <obo:RO_0001025 rdf:resource="http://purl.obolibrary.org/obo/GAZ_00052529"/>
        <obo:RO_0001025 rdf:resource="http://purl.obolibrary.org/obo/GAZ_00052531"/>
        <obo:IAO_0000115>A populated place. A village in south-central Ethiopia. Located in the Bale Zone of the Oromia Region in the heart of the Bale Mountains.</obo:IAO_0000115>
        <oboInOwl:hasOBONamespace>GAZ</oboInOwl:hasOBONamespace>
        <oboInOwl:id>GAZ:00052530</oboInOwl:id>
        <rdfs:label>Dinsho</rdfs:label>
    </owl:NamedIndividual>
    


    <!-- http://purl.obolibrary.org/obo/GAZ_00052531 -->

    <owl:NamedIndividual rdf:about="http://purl.obolibrary.org/obo/GAZ_00052531">
        <rdf:type rdf:resource="http://purl.obolibrary.org/obo/ENVO_00000106"/>
        <obo:RO_0001025 rdf:resource="http://purl.obolibrary.org/obo/GAZ_00000784"/>
        <obo:RO_0001025 rdf:resource="http://purl.obolibrary.org/obo/GAZ_00123544"/>
        <obo:IAO_0000115>A range of mountains in the Oromia Region of southeast Ethiopia, south of the Awash River. They include Tullu Demtu, the second-highest mountain in Ethiopia (4377 m), and Mount Batu (4307 m). The Web River, a tributary of the Jubba River, rises in these mountains east of Goba.</obo:IAO_0000115>
        <oboInOwl:hasOBONamespace>GAZ</oboInOwl:hasOBONamespace>
        <oboInOwl:id>GAZ:00052531</oboInOwl:id>
        <rdfs:label>Bale Mountains</rdfs:label>
    </owl:NamedIndividual>
    


    <!-- http://purl.obolibrary.org/obo/GAZ_00052532 -->

    <owl:NamedIndividual rdf:about="http://purl.obolibrary.org/obo/GAZ_00052532">
        <obo:RO_0001025 rdf:resource="http://purl.obolibrary.org/obo/GAZ_00052531"/>
        <obo:RO_0001025 rdf:resource="http://purl.obolibrary.org/obo/GAZ_00123768"/>
        <obo:IAO_0000115>A national park in the Oromia Region of southeast Ethiopia. Created in 1970, this park covers about 2,200 km2 of the Bale Mountains to the west and southwest of Goba in the Bale Zone. Within its boundaries are some of the highest points in Ethiopia, which include Mount Batu. Bale Mountains contains three distinct ecoregions: the northern plains, bush and woods; the central Sanetti Plateau with an average elevation of over 4000 meters; and the southern Harenna Forest.</obo:IAO_0000115>
        <oboInOwl:hasOBONamespace>GAZ</oboInOwl:hasOBONamespace>
        <oboInOwl:id>GAZ:00052532</oboInOwl:id>
        <rdfs:label>Bale Mountains National Park</rdfs:label>
    </owl:NamedIndividual>
    


    <!-- http://purl.obolibrary.org/obo/GAZ_00052533 -->

    <owl:NamedIndividual rdf:about="http://purl.obolibrary.org/obo/GAZ_00052533">
        <obo:RO_0001025 rdf:resource="http://purl.obolibrary.org/obo/GAZ_00031093"/>
        <obo:IAO_0000115>A woreda in central Ethiopia. Located in the Semien Shewa Zone of the Amhara Region, about 120 km north east of Addis Ababa on the paved highway to Dessie. An enclave within Debre Berhan Zuria Woreda.</obo:IAO_0000115>
        <oboInOwl:hasOBONamespace>GAZ</oboInOwl:hasOBONamespace>
        <oboInOwl:id>GAZ:00052533</oboInOwl:id>
        <rdfs:label>Debre Berhan Woreda</rdfs:label>
    </owl:NamedIndividual>
    


    <!-- http://purl.obolibrary.org/obo/GAZ_00052534 -->

    <owl:NamedIndividual rdf:about="http://purl.obolibrary.org/obo/GAZ_00052534">
        <obo:RO_0001025 rdf:resource="http://purl.obolibrary.org/obo/GAZ_00052533"/>
        <obo:IAO_0000115>A populated place. A city in central Ethiopia. Located in the Semien Shewa Zone of the Amhara Region, about 120 km north east of Addis Ababa on the paved highway to Dessie.</obo:IAO_0000115>
        <oboInOwl:hasOBONamespace>GAZ</oboInOwl:hasOBONamespace>
        <oboInOwl:id>GAZ:00052534</oboInOwl:id>
        <rdfs:label>Debre Berhan</rdfs:label>
    </owl:NamedIndividual>
    


    <!-- http://purl.obolibrary.org/obo/GAZ_00052535 -->

    <owl:NamedIndividual rdf:about="http://purl.obolibrary.org/obo/GAZ_00052535">
        <obo:RO_0001025 rdf:resource="http://purl.obolibrary.org/obo/GAZ_00031101"/>
        <obo:IAO_0000115>One of the 105 woredas in the Amhara Region of Ethiopia. This woreda is named after the former district. Part of the Semien Wollo Zone, Bugna is bordered on the south by Meket, on the west by the Debub Gondar Zone, on the north by the Wag Hemra Zone, and on the east by Gidan. The major city in Bugna is Lalibela.</obo:IAO_0000115>
        <oboInOwl:hasOBONamespace>GAZ</oboInOwl:hasOBONamespace>
        <oboInOwl:id>GAZ:00052535</oboInOwl:id>
        <rdfs:label>Bugna Woreda</rdfs:label>
    </owl:NamedIndividual>
    


    <!-- http://purl.obolibrary.org/obo/GAZ_00052536 -->

    <owl:NamedIndividual rdf:about="http://purl.obolibrary.org/obo/GAZ_00052536">
        <rdf:type rdf:resource="http://purl.obolibrary.org/obo/ENVO_00000856"/>
        <obo:RO_0001025 rdf:resource="http://purl.obolibrary.org/obo/GAZ_00053681"/>
        <obo:IAO_0000115>A populated place. A town of Ethiopia, lying south east of Addis Ababa. It is known for five crater lakes: Lake Bishoftu, Lake Hora, Lake Bishoftu Guda, Lake Koriftu and the seasonal Lake Cheleklaka.</obo:IAO_0000115>
        <oboInOwl:hasOBONamespace>GAZ</oboInOwl:hasOBONamespace>
        <oboInOwl:id>GAZ:00052536</oboInOwl:id>
        <rdfs:label>Debre Zeyit</rdfs:label>
    </owl:NamedIndividual>
    


    <!-- http://purl.obolibrary.org/obo/GAZ_00052538 -->

    <owl:NamedIndividual rdf:about="http://purl.obolibrary.org/obo/GAZ_00052538">
        <rdf:type rdf:resource="http://purl.obolibrary.org/obo/ENVO_00000080"/>
        <obo:RO_0001025 rdf:resource="http://purl.obolibrary.org/obo/GAZ_00000784"/>
        <obo:IAO_0000115>A mountain chain immediately north of Addis Ababa, in the Oromia Region of Ethiopia.</obo:IAO_0000115>
        <oboInOwl:hasOBONamespace>GAZ</oboInOwl:hasOBONamespace>
        <oboInOwl:id>GAZ:00052538</oboInOwl:id>
        <rdfs:label>Entoto Mountains</rdfs:label>
    </owl:NamedIndividual>
    


    <!-- http://purl.obolibrary.org/obo/GAZ_00052539 -->

    <owl:NamedIndividual rdf:about="http://purl.obolibrary.org/obo/GAZ_00052539">
        <obo:RO_0001025 rdf:resource="http://purl.obolibrary.org/obo/GAZ_00052538"/>
        <obo:IAO_0000115>The highest peak overlooking the city of Addis Ababa, the capital of Ethiopia. Mount Entoto is part of the Entoto mountain chain, reaching 3,200 m above sea level.</obo:IAO_0000115>
        <oboInOwl:hasOBONamespace>GAZ</oboInOwl:hasOBONamespace>
        <oboInOwl:id>GAZ:00052539</oboInOwl:id>
        <rdfs:label>Mount Entoto</rdfs:label>
    </owl:NamedIndividual>
    


    <!-- http://purl.obolibrary.org/obo/GAZ_00052540 -->

    <owl:NamedIndividual rdf:about="http://purl.obolibrary.org/obo/GAZ_00052540">
        <obo:RO_0001025 rdf:resource="http://purl.obolibrary.org/obo/GAZ_00123427"/>
        <obo:RO_0001025 rdf:resource="http://purl.obolibrary.org/obo/GAZ_00123874"/>
        <obo:IAO_0000115>A national park located at the southern tip of the Afar Region, this park is 225 km east of Addis Ababa (and a few km west of Awash), with its southern boundary along the Awash River, and covers at least 756 km2 of acacia woodland and grassland.</obo:IAO_0000115>
        <oboInOwl:hasOBONamespace>GAZ</oboInOwl:hasOBONamespace>
        <oboInOwl:id>GAZ:00052540</oboInOwl:id>
        <rdfs:label>Awash National Park</rdfs:label>
    </owl:NamedIndividual>
    


    <!-- http://purl.obolibrary.org/obo/GAZ_00052541 -->

    <owl:NamedIndividual rdf:about="http://purl.obolibrary.org/obo/GAZ_00052541">
        <obo:RO_0001025 rdf:resource="http://purl.obolibrary.org/obo/GAZ_00052540"/>
        <oboInOwl:hasOBONamespace>GAZ</oboInOwl:hasOBONamespace>
        <oboInOwl:id>GAZ:00052541</oboInOwl:id>
        <rdfs:label>Kudu Valley</rdfs:label>
    </owl:NamedIndividual>
    


    <!-- http://purl.obolibrary.org/obo/GAZ_00052542 -->

    <owl:NamedIndividual rdf:about="http://purl.obolibrary.org/obo/GAZ_00052542">
        <obo:RO_0001025 rdf:resource="http://purl.obolibrary.org/obo/GAZ_00052541"/>
        <obo:IAO_0000115>Hot springs.</obo:IAO_0000115>
        <oboInOwl:hasOBONamespace>GAZ</oboInOwl:hasOBONamespace>
        <oboInOwl:id>GAZ:00052542</oboInOwl:id>
        <rdfs:label>Filwoha Hot Springs</rdfs:label>
    </owl:NamedIndividual>
    


    <!-- http://purl.obolibrary.org/obo/GAZ_00052543 -->

    <owl:NamedIndividual rdf:about="http://purl.obolibrary.org/obo/GAZ_00052543">
        <obo:RO_0001025 rdf:resource="http://purl.obolibrary.org/obo/GAZ_00052544"/>
        <obo:IAO_0000115>A populated place. A city in southwestern Ethiopia. Located in the Jimma Zone of the Oromia Region.</obo:IAO_0000115>
        <oboInOwl:hasOBONamespace>GAZ</oboInOwl:hasOBONamespace>
        <oboInOwl:id>GAZ:00052543</oboInOwl:id>
        <rdfs:label>Jimma</rdfs:label>
    </owl:NamedIndividual>
    


    <!-- http://purl.obolibrary.org/obo/GAZ_00052544 -->

    <owl:NamedIndividual rdf:about="http://purl.obolibrary.org/obo/GAZ_00052544">
        <obo:RO_0001025 rdf:resource="http://purl.obolibrary.org/obo/GAZ_00031118"/>
        <obo:IAO_0000115>One of the 180 woredas in the Oromia Region of Ethiopia. Part of the Jimma Zone, Kersa is bordered on the south by Dedo, on the southwest by Seka Chekorsa, on the west by Mana, on the north by Limmu Kosa, on the northeast by Tiro Afeta, and on the southeast by Omo Nada. Towns and cities in Kersa include Jimma, the Zonal capital, and Serbo.</obo:IAO_0000115>
        <oboInOwl:hasOBONamespace>GAZ</oboInOwl:hasOBONamespace>
        <oboInOwl:id>GAZ:00052544</oboInOwl:id>
        <rdfs:label>Kersa Woreda</rdfs:label>
    </owl:NamedIndividual>
    


    <!-- http://purl.obolibrary.org/obo/GAZ_00052547 -->

    <owl:NamedIndividual rdf:about="http://purl.obolibrary.org/obo/GAZ_00052547">
        <obo:RO_0001025 rdf:resource="http://purl.obolibrary.org/obo/GAZ_00000786"/>
        <obo:IAO_0000115>One of the 77 woredas in the Southern Nations, Nationalities, and Peoples Region (SNNPR) of Ethiopia. Because Konso is not part of any Zone in the SNNPR, it is considered a Special woreda. Located in the Great Rift Valley, Konso is bordered on the south by the Oromia Region, on the west by the Weito River which separates it from the Debub Omo Zone, on the north by the Dirashe Special Woreda, and on the east by Burji Special Woreda. The Sagan River, which flows south then west to join the Weito, defines part of the woreda&apos;s boundary with Burji and the entire length of the boundary with the Oromia Region. The administrative center is Karati; other towns in Konso include Fasha and Sagan. Rivers in this woreda include the Talpeena, a tributary of the Sagan.</obo:IAO_0000115>
        <oboInOwl:hasOBONamespace>GAZ</oboInOwl:hasOBONamespace>
        <oboInOwl:id>GAZ:00052547</oboInOwl:id>
        <rdfs:label>Konso Special Woreda</rdfs:label>
    </owl:NamedIndividual>
    


    <!-- http://purl.obolibrary.org/obo/GAZ_00052548 -->

    <owl:NamedIndividual rdf:about="http://purl.obolibrary.org/obo/GAZ_00052548">
        <rdf:type rdf:resource="http://purl.obolibrary.org/obo/ENVO_00000856"/>
        <obo:RO_0001025 rdf:resource="http://purl.obolibrary.org/obo/GAZ_00052547"/>
        <obo:IAO_0000115>A populated place. A town on the Sagan River in southwestern Ethiopia.</obo:IAO_0000115>
        <oboInOwl:hasOBONamespace>GAZ</oboInOwl:hasOBONamespace>
        <oboInOwl:id>GAZ:00052548</oboInOwl:id>
        <rdfs:label>Konso</rdfs:label>
    </owl:NamedIndividual>
    


    <!-- http://purl.obolibrary.org/obo/GAZ_00052549 -->

    <owl:NamedIndividual rdf:about="http://purl.obolibrary.org/obo/GAZ_00052549">
        <obo:RO_0001025 rdf:resource="http://purl.obolibrary.org/obo/GAZ_00031151"/>
        <obo:IAO_0000115>One of the 36 woredas in the Tigray Region of Ethiopia. Part of the Misraqawi Zone, Wukro is bordered on the south by the Debubawi (Southern) Zone, on the west by the Mehakelegnaw (Central) Zone, on the north by Hawzen, and on the east by Atsbi Wenberta. Towns in Wukro include Agula, Tsigereda and Wukro.</obo:IAO_0000115>
        <oboInOwl:hasOBONamespace>GAZ</oboInOwl:hasOBONamespace>
        <oboInOwl:id>GAZ:00052549</oboInOwl:id>
        <rdfs:label>Wukro Woreda</rdfs:label>
    </owl:NamedIndividual>
    


    <!-- http://purl.obolibrary.org/obo/GAZ_00052550 -->

    <owl:NamedIndividual rdf:about="http://purl.obolibrary.org/obo/GAZ_00052550">
        <obo:RO_0001025 rdf:resource="http://purl.obolibrary.org/obo/GAZ_00052549"/>
        <obo:RO_0001025 rdf:resource="http://purl.obolibrary.org/obo/GAZ_00052552"/>
        <oboInOwl:hasOBONamespace>GAZ</oboInOwl:hasOBONamespace>
        <oboInOwl:id>GAZ:00052550</oboInOwl:id>
        <rdfs:label>Korir Dam</rdfs:label>
    </owl:NamedIndividual>
    


    <!-- http://purl.obolibrary.org/obo/GAZ_00052551 -->

    <owl:NamedIndividual rdf:about="http://purl.obolibrary.org/obo/GAZ_00052551">
        <obo:RO_0001025 rdf:resource="http://purl.obolibrary.org/obo/GAZ_00052549"/>
        <obo:RO_0001025 rdf:resource="http://purl.obolibrary.org/obo/GAZ_00052552"/>
        <oboInOwl:hasOBONamespace>GAZ</oboInOwl:hasOBONamespace>
        <oboInOwl:id>GAZ:00052551</oboInOwl:id>
        <rdfs:label>Laelay Wukro Dam</rdfs:label>
    </owl:NamedIndividual>
    


    <!-- http://purl.obolibrary.org/obo/GAZ_00052552 -->

    <owl:NamedIndividual rdf:about="http://purl.obolibrary.org/obo/GAZ_00052552">
        <obo:RO_0001025 rdf:resource="http://purl.obolibrary.org/obo/GAZ_00000567"/>
        <obo:IAO_0000115>A river basin in Ethiopia.</obo:IAO_0000115>
        <oboInOwl:hasOBONamespace>GAZ</oboInOwl:hasOBONamespace>
        <oboInOwl:id>GAZ:00052552</oboInOwl:id>
        <rdfs:label>Tekeze River Basin</rdfs:label>
    </owl:NamedIndividual>
    


    <!-- http://purl.obolibrary.org/obo/GAZ_00052553 -->

    <owl:NamedIndividual rdf:about="http://purl.obolibrary.org/obo/GAZ_00052553">
        <obo:RO_0001025 rdf:resource="http://purl.obolibrary.org/obo/GAZ_00052552"/>
        <obo:IAO_0000115>A river that rises in the central highlands of Ethiopia near Mount Qachen, from where it flows west, north, then west again, forming the westernmost border of Ethiopia and Eritrea. The river continues into northeastern Sudan, where at 14deg10minN, 36degE, the Tekeze joins the Atbarah River, the lower course of which is a tributary of the Nile. The Tekeze is perhaps the true upper course of the Atbarah, as the former follows the longer course prior to the confluence of the two rivers. The names of its main tributaries in Ethiopia from its source are: on the right bank Tahali, Meri, Sellare, Sullo, Arekwa, Gheoa, Wari, Firafira, Tocoro and Gumalo Rivers; on the left bank Nili, Balagas, Saha, Bembea, Ataba, Zarima, and Kwalema Rivers.</obo:IAO_0000115>
        <oboInOwl:hasOBONamespace>GAZ</oboInOwl:hasOBONamespace>
        <oboInOwl:id>GAZ:00052553</oboInOwl:id>
        <rdfs:label>Tekeze River</rdfs:label>
    </owl:NamedIndividual>
    


    <!-- http://purl.obolibrary.org/obo/GAZ_00052554 -->

    <owl:NamedIndividual rdf:about="http://purl.obolibrary.org/obo/GAZ_00052554">
        <obo:RO_0001025 rdf:resource="http://purl.obolibrary.org/obo/GAZ_00031119"/>
        <obo:IAO_0000115>One of the 180 woredas in the Oromia Region of Ethiopia. It is named after the woreda capital Adama, also known as Nazaret. Other towns include Awash Melkasa, Shewa Alemtena, Sire Robi, Sodere and Wenji Gefersa. Part of the Misraq Shewa Zone located in the Great Rift Valley, Adama is bordered on the south by the Arsi Zone, on the southwest by Koka Reservoir which separates it from Dugda Bora, on the west by Lome, on the north by the Afar Region, and on the east by Boset; the Awash River, the only important river in this woreda, defines the woreda boundaries on the east and south.</obo:IAO_0000115>
        <oboInOwl:hasOBONamespace>GAZ</oboInOwl:hasOBONamespace>
        <oboInOwl:id>GAZ:00052554</oboInOwl:id>
        <rdfs:label>Adama Woreda</rdfs:label>
    </owl:NamedIndividual>
    


    <!-- http://purl.obolibrary.org/obo/GAZ_00052555 -->

    <owl:NamedIndividual rdf:about="http://purl.obolibrary.org/obo/GAZ_00052555">
        <obo:RO_0001025 rdf:resource="http://purl.obolibrary.org/obo/GAZ_00052554"/>
        <obo:IAO_0000115>A populated place. A city in Ethiopia and the current capital of the Oromia Region.</obo:IAO_0000115>
        <oboInOwl:hasOBONamespace>GAZ</oboInOwl:hasOBONamespace>
        <oboInOwl:id>GAZ:00052555</oboInOwl:id>
        <rdfs:label>Adama</rdfs:label>
    </owl:NamedIndividual>
    


    <!-- http://purl.obolibrary.org/obo/GAZ_00052556 -->

    <owl:NamedIndividual rdf:about="http://purl.obolibrary.org/obo/GAZ_00052556">
        <obo:RO_0001025 rdf:resource="http://purl.obolibrary.org/obo/GAZ_00052555"/>
        <obo:IAO_0000115>An agricultural research center.</obo:IAO_0000115>
        <oboInOwl:hasOBONamespace>GAZ</oboInOwl:hasOBONamespace>
        <oboInOwl:id>GAZ:00052556</oboInOwl:id>
        <rdfs:label>Ethiopian Institute of Agricultural Research Melkassa Research Centre</rdfs:label>
    </owl:NamedIndividual>
    


    <!-- http://purl.obolibrary.org/obo/GAZ_00052557 -->

    <owl:NamedIndividual rdf:about="http://purl.obolibrary.org/obo/GAZ_00052557">
        <obo:RO_0001025 rdf:resource="http://purl.obolibrary.org/obo/GAZ_00000785"/>
        <obo:IAO_0000115>A part of the Somali Regional State in Ethiopia. The area which is around 200,000 km2, borders Djibouti, Kenya, and Somalia. Important settlements include Degehabur (Dhagaxbuur in Somali), Gode (Godey), Jijiga (Jigjiga), Kebri Dahar (Qabridahare), Shilavo (Shilaabo) and Werder (Wardheer).</obo:IAO_0000115>
        <oboInOwl:hasOBONamespace>GAZ</oboInOwl:hasOBONamespace>
        <oboInOwl:id>GAZ:00052557</oboInOwl:id>
        <rdfs:label>Ogaden</rdfs:label>
    </owl:NamedIndividual>
    


    <!-- http://purl.obolibrary.org/obo/GAZ_00052558 -->

    <owl:NamedIndividual rdf:about="http://purl.obolibrary.org/obo/GAZ_00052558">
        <obo:RO_0001025 rdf:resource="http://purl.obolibrary.org/obo/GAZ_00031096"/>
        <obo:IAO_0000115>A populated place. A city in north western Ethiopia, and the capital of the Amhara Region.</obo:IAO_0000115>
        <oboInOwl:hasOBONamespace>GAZ</oboInOwl:hasOBONamespace>
        <oboInOwl:id>GAZ:00052558</oboInOwl:id>
        <rdfs:label>Bahir Dar</rdfs:label>
    </owl:NamedIndividual>
    


    <!-- http://purl.obolibrary.org/obo/GAZ_00052559 -->

    <owl:NamedIndividual rdf:about="http://purl.obolibrary.org/obo/GAZ_00052559">
        <rdf:type rdf:resource="http://purl.obolibrary.org/obo/ENVO_00000191"/>
        <obo:RO_0001025 rdf:resource="http://purl.obolibrary.org/obo/GAZ_00052532"/>
        <obo:IAO_0000115>A major landform in Ethopia within a portion of the Bale Mountains.</obo:IAO_0000115>
        <oboInOwl:hasOBONamespace>GAZ</oboInOwl:hasOBONamespace>
        <oboInOwl:id>GAZ:00052559</oboInOwl:id>
        <rdfs:label>Sanetti Plateau</rdfs:label>
    </owl:NamedIndividual>
    


    <!-- http://purl.obolibrary.org/obo/GAZ_00052562 -->

    <owl:NamedIndividual rdf:about="http://purl.obolibrary.org/obo/GAZ_00052562">
        <obo:RO_0001025 rdf:resource="http://purl.obolibrary.org/obo/GAZ_00031122"/>
        <obo:IAO_0000115>One of the 180 woredas in the Oromia Region of Ethiopia. Part of the Semien Shewa Zone, Mulona Sululta is bordered on the south by the city of Addis Ababa, on the west by the Muger River which separates it from the Mirab Shewa Zone, on the north by Yaya Gulelena Debre Liban, on the northeast by Wuchalena Jido, and on the east by Berehna Aleltu. Towns in Mulona Sululta include Chancho, Derba, Muger Sheleko, Rob Gebeya, Sululta and Segno Gebeya.</obo:IAO_0000115>
        <oboInOwl:hasOBONamespace>GAZ</oboInOwl:hasOBONamespace>
        <oboInOwl:id>GAZ:00052562</oboInOwl:id>
        <rdfs:label>Mulona Sululta Woreda</rdfs:label>
    </owl:NamedIndividual>
    


    <!-- http://purl.obolibrary.org/obo/GAZ_00052563 -->

    <owl:NamedIndividual rdf:about="http://purl.obolibrary.org/obo/GAZ_00052563">
        <obo:RO_0001025 rdf:resource="http://purl.obolibrary.org/obo/GAZ_00052562"/>
        <obo:IAO_0000115>A populated place.</obo:IAO_0000115>
        <oboInOwl:hasOBONamespace>GAZ</oboInOwl:hasOBONamespace>
        <oboInOwl:id>GAZ:00052563</oboInOwl:id>
        <rdfs:label>Sululta</rdfs:label>
    </owl:NamedIndividual>
    


    <!-- http://purl.obolibrary.org/obo/GAZ_00052564 -->

    <owl:NamedIndividual rdf:about="http://purl.obolibrary.org/obo/GAZ_00052564">
        <obo:RO_0001025 rdf:resource="http://purl.obolibrary.org/obo/GAZ_00031143"/>
        <obo:IAO_0000115>One of the 77 woredas in the Southern Nations, Nationalities and Peoples&apos; Region of Ethiopia. Part of the Debub Omo Zone, Hamer Bena is bordered on the south by Kenya, on the southwest by Kuraz, on the northwest by the Usno River which separates it from Selamago, on the north by Bako Gazer, on the northeast by the Konso special woreda, and on the east by the Oromia Region; the Weito River separates it from Konso and the Oromia Region and the Neri River defines part of the boundary with Bako Gazer. Hamer Bena includes part of Lake Chew Bahir along its southeastern border. Towns in Hamer Bena include Arbore and Turmi.</obo:IAO_0000115>
        <oboInOwl:hasOBONamespace>GAZ</oboInOwl:hasOBONamespace>
        <oboInOwl:id>GAZ:00052564</oboInOwl:id>
        <rdfs:label>Hamer Bena Woreda</rdfs:label>
    </owl:NamedIndividual>
    


    <!-- http://purl.obolibrary.org/obo/GAZ_00052565 -->

    <owl:NamedIndividual rdf:about="http://purl.obolibrary.org/obo/GAZ_00052565">
        <obo:RO_0001025 rdf:resource="http://purl.obolibrary.org/obo/GAZ_00052564"/>
        <obo:IAO_0000115>A populated place. A market town in southwestern Ethiopia. Located in the Debub Omo Zone of the Southern Nations, Nationalities, and People&apos;s Region.</obo:IAO_0000115>
        <oboInOwl:hasOBONamespace>GAZ</oboInOwl:hasOBONamespace>
        <oboInOwl:id>GAZ:00052565</oboInOwl:id>
        <rdfs:label>Turmi</rdfs:label>
    </owl:NamedIndividual>
    


    <!-- http://purl.obolibrary.org/obo/GAZ_00052566 -->

    <owl:NamedIndividual rdf:about="http://purl.obolibrary.org/obo/GAZ_00052566">
        <obo:RO_0001025 rdf:resource="http://purl.obolibrary.org/obo/GAZ_00052564"/>
        <obo:RO_0001025 rdf:resource="http://purl.obolibrary.org/obo/GAZ_00123622"/>
        <obo:RO_0001025 rdf:resource="http://purl.obolibrary.org/obo/GAZ_00123623"/>
        <obo:RO_0001025 rdf:resource="http://purl.obolibrary.org/obo/GAZ_00123652"/>
        <obo:RO_0001025 rdf:resource="http://purl.obolibrary.org/obo/GAZ_00123683"/>
        <obo:IAO_0000115>A national park located in the Southern Nations, Nationalities, and Peoples Region on the west bank of the Omo River, the park covers approximately 4,068 km2.</obo:IAO_0000115>
        <oboInOwl:hasOBONamespace>GAZ</oboInOwl:hasOBONamespace>
        <oboInOwl:id>GAZ:00052566</oboInOwl:id>
        <rdfs:label>Omo National Park</rdfs:label>
    </owl:NamedIndividual>
    


    <!-- http://purl.obolibrary.org/obo/GAZ_00052567 -->

    <owl:NamedIndividual rdf:about="http://purl.obolibrary.org/obo/GAZ_00052567">
        <obo:RO_0001025 rdf:resource="http://purl.obolibrary.org/obo/GAZ_00000567"/>
        <obo:IAO_0000115>A river of southern Ethiopia. Its course is entirely contained within the boundaries of Ethiopia, and empties into Lake Turkana on the border with Kenya. It is the principal stream of an endorheic drainage basin; the part that the Omo drains includes part of the western Oromia Region and the middle of the Southern Nations, Nationalities, and People&apos;s Region. This river rises in the Shewan highlands and is a perennial river. Its course is generally to the south, however with a major bend to the west at about 7deg N 37deg 30minE to about 36deg E where it turns south until 5deg 30min N where it makes a large S- bend then resumes its southernly course to Lake Turkana.</obo:IAO_0000115>
        <oboInOwl:hasOBONamespace>GAZ</oboInOwl:hasOBONamespace>
        <oboInOwl:id>GAZ:00052567</oboInOwl:id>
        <rdfs:label>Omo River</rdfs:label>
    </owl:NamedIndividual>
    


    <!-- http://purl.obolibrary.org/obo/GAZ_00052568 -->

    <owl:NamedIndividual rdf:about="http://purl.obolibrary.org/obo/GAZ_00052568">
        <obo:RO_0001025 rdf:resource="http://purl.obolibrary.org/obo/GAZ_00031139"/>
        <obo:IAO_0000115>One of the 77 woredas in the Southern Nations, Nationalities and Peoples&apos; Region (SNNPR) of Ethiopia. Part of the Sidama Zone located in the Great Rift Valley, Awasa is bordered on the south by Shebedino, and on the west, north and east by the Oromia Region. This woreda almost surrounds Lake Awasa on all sides. Towns and cities in Awasa include Awasa, the capital of the Southern Nations, Nationalities, and Peoples Region, and Wendo Genet.</obo:IAO_0000115>
        <oboInOwl:hasOBONamespace>GAZ</oboInOwl:hasOBONamespace>
        <oboInOwl:id>GAZ:00052568</oboInOwl:id>
        <rdfs:label>Awasa Woreda</rdfs:label>
    </owl:NamedIndividual>
    


    <!-- http://purl.obolibrary.org/obo/GAZ_00052569 -->

    <owl:NamedIndividual rdf:about="http://purl.obolibrary.org/obo/GAZ_00052569">
        <obo:RO_0001025 rdf:resource="http://purl.obolibrary.org/obo/GAZ_00052568"/>
        <obo:IAO_0000115>A populated place. A city in Ethiopia, on the shores of Lake Awasa in the Great Rift Valley.</obo:IAO_0000115>
        <oboInOwl:hasOBONamespace>GAZ</oboInOwl:hasOBONamespace>
        <oboInOwl:id>GAZ:00052569</oboInOwl:id>
        <rdfs:label>Awasa</rdfs:label>
    </owl:NamedIndividual>
    


    <!-- http://purl.obolibrary.org/obo/GAZ_00052571 -->

    <owl:NamedIndividual rdf:about="http://purl.obolibrary.org/obo/GAZ_00052571">
        <obo:RO_0001025 rdf:resource="http://purl.obolibrary.org/obo/GAZ_00123575"/>
        <obo:IAO_0000115>A populated place.</obo:IAO_0000115>
        <oboInOwl:hasOBONamespace>GAZ</oboInOwl:hasOBONamespace>
        <oboInOwl:id>GAZ:00052571</oboInOwl:id>
        <rdfs:label>Coccia</rdfs:label>
    </owl:NamedIndividual>
    


    <!-- http://purl.obolibrary.org/obo/GAZ_00052573 -->

    <owl:NamedIndividual rdf:about="http://purl.obolibrary.org/obo/GAZ_00052573">
        <obo:RO_0001025 rdf:resource="http://purl.obolibrary.org/obo/GAZ_00031099"/>
        <obo:IAO_0000115>A woreda located in the Semien Gondar Zone of the Amhara Region, Gondar is north of Lake Tana on the Lesser Angereb River and southwest of the Simien Mountains. An enclave within Gondar Zuria Woreda.</obo:IAO_0000115>
        <oboInOwl:hasOBONamespace>GAZ</oboInOwl:hasOBONamespace>
        <oboInOwl:id>GAZ:00052573</oboInOwl:id>
        <rdfs:label>Gondar Woreda</rdfs:label>
    </owl:NamedIndividual>
    


    <!-- http://purl.obolibrary.org/obo/GAZ_00052574 -->

    <owl:NamedIndividual rdf:about="http://purl.obolibrary.org/obo/GAZ_00052574">
        <obo:RO_0001025 rdf:resource="http://purl.obolibrary.org/obo/GAZ_00052573"/>
        <obo:IAO_0000115>A populated place. A city in Ethiopia, which was once the old imperial capital and capital of the historic Begemder province. As a result, the old province of Begemder is sometimes referred to as Gondar. Located in the Semien Gondar Zone of the Amhara Region, Gondar is north of Lake Tana on the Lesser Angereb River and southwest of the Simien Mountains.</obo:IAO_0000115>
        <oboInOwl:hasOBONamespace>GAZ</oboInOwl:hasOBONamespace>
        <oboInOwl:id>GAZ:00052574</oboInOwl:id>
        <rdfs:label>Gondar</rdfs:label>
    </owl:NamedIndividual>
    


    <!-- http://purl.obolibrary.org/obo/GAZ_00052576 -->

    <owl:NamedIndividual rdf:about="http://purl.obolibrary.org/obo/GAZ_00052576">
        <rdf:type rdf:resource="http://purl.obolibrary.org/obo/ENVO_00000856"/>
        <obo:RO_0001025 rdf:resource="http://purl.obolibrary.org/obo/GAZ_00052577"/>
        <obo:IAO_0000115>A populated place. A town in southern Ethiopia. An alternative name for this town is Obda, which is also the name of a nearby mountain. Located northwest of Moyale in the Borena Zone of the Oromia Region.</obo:IAO_0000115>
        <oboInOwl:hasOBONamespace>GAZ</oboInOwl:hasOBONamespace>
        <oboInOwl:id>GAZ:00052576</oboInOwl:id>
        <rdfs:label>Yabelo</rdfs:label>
    </owl:NamedIndividual>
    


    <!-- http://purl.obolibrary.org/obo/GAZ_00052577 -->

    <owl:NamedIndividual rdf:about="http://purl.obolibrary.org/obo/GAZ_00052577">
        <obo:RO_0001025 rdf:resource="http://purl.obolibrary.org/obo/GAZ_00031113"/>
        <obo:IAO_0000115>One of the 180 woredas in the Oromia Region of Ethiopia. It is named after the administrative center, Yabelo. Part of the Borena Zone, Yabelo is bordered on the south by Dire, on the west by Teltele, on the north by Hagere Mariam, and on the east by Arero.</obo:IAO_0000115>
        <oboInOwl:hasOBONamespace>GAZ</oboInOwl:hasOBONamespace>
        <oboInOwl:id>GAZ:00052577</oboInOwl:id>
        <rdfs:label>Yabelo Woreda</rdfs:label>
    </owl:NamedIndividual>
    


    <!-- http://purl.obolibrary.org/obo/GAZ_00052578 -->

    <owl:NamedIndividual rdf:about="http://purl.obolibrary.org/obo/GAZ_00052578">
        <obo:RO_0001025 rdf:resource="http://purl.obolibrary.org/obo/GAZ_00031101"/>
        <obo:RO_0001025 rdf:resource="http://purl.obolibrary.org/obo/GAZ_00123532"/>
        <obo:RO_0001025 rdf:resource="http://purl.obolibrary.org/obo/GAZ_00123534"/>
        <obo:RO_0001025 rdf:resource="http://purl.obolibrary.org/obo/GAZ_00123535"/>
        <obo:RO_0001025 rdf:resource="http://purl.obolibrary.org/obo/GAZ_00123539"/>
        <obo:RO_0001025 rdf:resource="http://purl.obolibrary.org/obo/GAZ_00123543"/>
        <obo:IAO_0000115>Mountains in northern Ethiopia, north east of Gondar. The mountains consist of plateaux separated by valleys and rising to pinnacles. The tallest peak is Ras Dashen (4,543 m); other notable heights include Mounts Biuat (4,437 m) and Abba Yared (4,460 m).</obo:IAO_0000115>
        <oboInOwl:hasOBONamespace>GAZ</oboInOwl:hasOBONamespace>
        <oboInOwl:id>GAZ:00052578</oboInOwl:id>
        <rdfs:label>Semien Mountains</rdfs:label>
    </owl:NamedIndividual>
    


    <!-- http://purl.obolibrary.org/obo/GAZ_00052683 -->

    <owl:NamedIndividual rdf:about="http://purl.obolibrary.org/obo/GAZ_00052683">
        <obo:RO_0001025 rdf:resource="http://purl.obolibrary.org/obo/GAZ_00051205"/>
        <obo:RO_0001025 rdf:resource="http://purl.obolibrary.org/obo/GAZ_00123407"/>
        <obo:IAO_0000115>A saline lake in the northern end of the Afar Depression, Ethiopia.</obo:IAO_0000115>
        <oboInOwl:hasOBONamespace>GAZ</oboInOwl:hasOBONamespace>
        <oboInOwl:id>GAZ:00052683</oboInOwl:id>
        <rdfs:label>Lake Karum</rdfs:label>
    </owl:NamedIndividual>
    


    <!-- http://purl.obolibrary.org/obo/GAZ_00052684 -->

    <owl:NamedIndividual rdf:about="http://purl.obolibrary.org/obo/GAZ_00052684">
        <obo:RO_0001025 rdf:resource="http://purl.obolibrary.org/obo/GAZ_00051205"/>
        <obo:IAO_0000115>A saline crater lake in central Djibouti, located at the southern border of Tadjoura Region, touching Dikhil Region. Fed by subterranean inflows which include infiltration of sea water, as well as by wadis which lead into the depression.</obo:IAO_0000115>
        <oboInOwl:hasOBONamespace>GAZ</oboInOwl:hasOBONamespace>
        <oboInOwl:id>GAZ:00052684</oboInOwl:id>
        <rdfs:label>Lake Asal</rdfs:label>
    </owl:NamedIndividual>
    


    <!-- http://purl.obolibrary.org/obo/GAZ_00052883 -->

    <owl:NamedIndividual rdf:about="http://purl.obolibrary.org/obo/GAZ_00052883">
        <obo:IAO_0000115>A dam on the Yarmuk River.</obo:IAO_0000115>
        <oboInOwl:hasOBONamespace>GAZ</oboInOwl:hasOBONamespace>
        <oboInOwl:id>GAZ:00052883</oboInOwl:id>
        <rdfs:label>Maqarin Dam</rdfs:label>
    </owl:NamedIndividual>
    


    <!-- http://purl.obolibrary.org/obo/GAZ_00052895 -->

    <owl:NamedIndividual rdf:about="http://purl.obolibrary.org/obo/GAZ_00052895">
        <obo:RO_0001025 rdf:resource="http://purl.obolibrary.org/obo/GAZ_00015452"/>
        <obo:IAO_0000115>A significant extension of northeastern Lake Victoria into western Kenya. It is a shallow inlet and is connected to the main lake by Rusinga Channel (3 mi wide), which is partly masked from the main body of the lake by islands. The port of Kisumu, Kenya&apos;s fourth largest city, stands on its northeastern shore.</obo:IAO_0000115>
        <oboInOwl:hasOBONamespace>GAZ</oboInOwl:hasOBONamespace>
        <oboInOwl:id>GAZ:00052895</oboInOwl:id>
        <rdfs:label>Winam Gulf</rdfs:label>
    </owl:NamedIndividual>
    


    <!-- http://purl.obolibrary.org/obo/GAZ_00052896 -->

    <owl:NamedIndividual rdf:about="http://purl.obolibrary.org/obo/GAZ_00052896">
        <obo:RO_0001025 rdf:resource="http://purl.obolibrary.org/obo/GAZ_00052895"/>
        <oboInOwl:hasOBONamespace>GAZ</oboInOwl:hasOBONamespace>
        <oboInOwl:id>GAZ:00052896</oboInOwl:id>
        <rdfs:label>Asembo Bay</rdfs:label>
    </owl:NamedIndividual>
    


    <!-- http://purl.obolibrary.org/obo/GAZ_00052899 -->

    <owl:NamedIndividual rdf:about="http://purl.obolibrary.org/obo/GAZ_00052899">
        <obo:RO_0001025 rdf:resource="http://purl.obolibrary.org/obo/GAZ_00007523"/>
        <oboInOwl:hasOBONamespace>GAZ</oboInOwl:hasOBONamespace>
        <oboInOwl:id>GAZ:00052899</oboInOwl:id>
        <rdfs:label>Causeway Pond</rdfs:label>
    </owl:NamedIndividual>
    


    <!-- http://purl.obolibrary.org/obo/GAZ_00052911 -->

    <owl:NamedIndividual rdf:about="http://purl.obolibrary.org/obo/GAZ_00052911">
        <obo:RO_0001025 rdf:resource="http://purl.obolibrary.org/obo/GAZ_00052895"/>
        <obo:IAO_0000115>A bay on the south shore of Winam Gulf of Lake Victoria, in western Kenya.</obo:IAO_0000115>
        <oboInOwl:hasOBONamespace>GAZ</oboInOwl:hasOBONamespace>
        <oboInOwl:id>GAZ:00052911</oboInOwl:id>
        <rdfs:label>Homa Bay</rdfs:label>
    </owl:NamedIndividual>
    


    <!-- http://purl.obolibrary.org/obo/GAZ_00052985 -->

    <owl:NamedIndividual rdf:about="http://purl.obolibrary.org/obo/GAZ_00052985">
        <obo:RO_0001025 rdf:resource="http://purl.obolibrary.org/obo/GAZ_00000007"/>
        <oboInOwl:hasOBONamespace>GAZ</oboInOwl:hasOBONamespace>
        <oboInOwl:id>GAZ:00052985</oboInOwl:id>
        <rdfs:label>Laikipia Plateau</rdfs:label>
    </owl:NamedIndividual>
    


    <!-- http://purl.obolibrary.org/obo/GAZ_00052986 -->

    <owl:NamedIndividual rdf:about="http://purl.obolibrary.org/obo/GAZ_00052986">
        <obo:RO_0001025 rdf:resource="http://purl.obolibrary.org/obo/GAZ_00052985"/>
        <obo:IAO_0000115>A research center.</obo:IAO_0000115>
        <oboInOwl:hasOBONamespace>GAZ</oboInOwl:hasOBONamespace>
        <oboInOwl:id>GAZ:00052986</oboInOwl:id>
        <rdfs:label>Mpala Research Centre</rdfs:label>
    </owl:NamedIndividual>
    


    <!-- http://purl.obolibrary.org/obo/GAZ_00053546 -->

    <owl:NamedIndividual rdf:about="http://purl.obolibrary.org/obo/GAZ_00053546">
        <obo:RO_0001025 rdf:resource="http://purl.obolibrary.org/obo/GAZ_00000007"/>
        <obo:IAO_0000115>A volcanic complex separates Lake Turkana from the broad Suguta Trough to the south, the site of a former lake. The volcano is comprised of four overlapping shield volcanoes, with the youngest, Kakorinya, located over the axis of the East African Rift. Kalolenyang volcano lies west of Kakorinya, and Likaiu West and Likaiu East volcano are located to the ENE. A 3.8 km wide summit caldera was formed at Kakorinya volcano about 92,000 years ago. Youthful-looking trachytic and phonolitic lava domes and flows erupted within the caldera and along its ring fracture fill much of the caldera floor. Early Holocene fissure-related scoria cones and lava flows dot the volcano&apos;s southern and northern flanks. Solfataric fields are located within the caldera and on the western and southern flanks of the volcano.</obo:IAO_0000115>
        <oboInOwl:hasOBONamespace>GAZ</oboInOwl:hasOBONamespace>
        <oboInOwl:id>GAZ:00053546</oboInOwl:id>
        <rdfs:label>The Barrier Volcanic Complex</rdfs:label>
    </owl:NamedIndividual>
    


    <!-- http://purl.obolibrary.org/obo/GAZ_00053547 -->

    <owl:NamedIndividual rdf:about="http://purl.obolibrary.org/obo/GAZ_00053547">
        <obo:RO_0001025 rdf:resource="http://purl.obolibrary.org/obo/GAZ_00053546"/>
        <obo:IAO_0000115>A volcano in the Barrier Complex.</obo:IAO_0000115>
        <oboInOwl:hasOBONamespace>GAZ</oboInOwl:hasOBONamespace>
        <oboInOwl:id>GAZ:00053547</oboInOwl:id>
        <rdfs:label>Kakorinya Volcano</rdfs:label>
    </owl:NamedIndividual>
    


    <!-- http://purl.obolibrary.org/obo/GAZ_00053548 -->

    <owl:NamedIndividual rdf:about="http://purl.obolibrary.org/obo/GAZ_00053548">
        <obo:RO_0001025 rdf:resource="http://purl.obolibrary.org/obo/GAZ_00053546"/>
        <obo:IAO_0000115>A volcano in the Barrier Complex.</obo:IAO_0000115>
        <oboInOwl:hasOBONamespace>GAZ</oboInOwl:hasOBONamespace>
        <oboInOwl:id>GAZ:00053548</oboInOwl:id>
        <rdfs:label>Likaiu East Volcano</rdfs:label>
    </owl:NamedIndividual>
    


    <!-- http://purl.obolibrary.org/obo/GAZ_00053549 -->

    <owl:NamedIndividual rdf:about="http://purl.obolibrary.org/obo/GAZ_00053549">
        <obo:RO_0001025 rdf:resource="http://purl.obolibrary.org/obo/GAZ_00053546"/>
        <obo:IAO_0000115>A volcano in the Barrier Complex.</obo:IAO_0000115>
        <oboInOwl:hasOBONamespace>GAZ</oboInOwl:hasOBONamespace>
        <oboInOwl:id>GAZ:00053549</oboInOwl:id>
        <rdfs:label>Kakorinya Volcano</rdfs:label>
    </owl:NamedIndividual>
    


    <!-- http://purl.obolibrary.org/obo/GAZ_00053550 -->

    <owl:NamedIndividual rdf:about="http://purl.obolibrary.org/obo/GAZ_00053550">
        <obo:RO_0001025 rdf:resource="http://purl.obolibrary.org/obo/GAZ_00053546"/>
        <obo:IAO_0000115>A volcano in the Barrier Complex.</obo:IAO_0000115>
        <oboInOwl:hasOBONamespace>GAZ</oboInOwl:hasOBONamespace>
        <oboInOwl:id>GAZ:00053550</oboInOwl:id>
        <rdfs:label>Likaiu West Volcano</rdfs:label>
    </owl:NamedIndividual>
    


    <!-- http://purl.obolibrary.org/obo/GAZ_00053551 -->

    <owl:NamedIndividual rdf:about="http://purl.obolibrary.org/obo/GAZ_00053551">
        <obo:RO_0001025 rdf:resource="http://purl.obolibrary.org/obo/GAZ_00000007"/>
        <obo:IAO_0000115>A trachytic shield volcano is topped by parasitic cones and lava flows of upper Pleistocene and Holocene age. Voluminous basaltic effusive and explosive activity took place during the early Holocene on the lower northern, eastern, and southern flanks along the axis of the East African Rift, producing fissure-controlled subaerial basaltic scoria cones and lava flows, and partially or completely sublacustral tuff cones, tuff rings, and pillow lavas. Fluid olivine basalts were also erupted from a breached scoria cone forming the summit of Namarunu.</obo:IAO_0000115>
        <oboInOwl:hasOBONamespace>GAZ</oboInOwl:hasOBONamespace>
        <oboInOwl:id>GAZ:00053551</oboInOwl:id>
        <rdfs:label>Namarunu Volcano</rdfs:label>
    </owl:NamedIndividual>
    


    <!-- http://purl.obolibrary.org/obo/GAZ_00053554 -->

    <owl:NamedIndividual rdf:about="http://purl.obolibrary.org/obo/GAZ_00053554">
        <obo:RO_0001025 rdf:resource="http://purl.obolibrary.org/obo/GAZ_00000007"/>
        <obo:IAO_0000115>A shield volcano is situated at a narrow constriction in the Rift Valley and almost completely straddles it. A 5 x 3.5 km summit caldera formed about 38,000 years ago. Since then trachytic and basaltic lava flows were erupted on the northern and southern flanks and within the caldera. A NNE-SSW-trending chain of lake-filled basaltic maars extends along the floor of the rift from the lower flanks of the volcano. Young lava flows were also erupted from vents along rift valley faults. Well-preserved parasitic cones erupted along rift-parallel faults cutting the volcano abound; the latest eruption produced a trachytic lava flow dated from secular magnetic variation measurements at about the beginning of the 20th century. Fumarolic activity and hot steaming ground occurs along NNE-trending fissures within the caldera and along the lower NW flanks.</obo:IAO_0000115>
        <oboInOwl:hasOBONamespace>GAZ</oboInOwl:hasOBONamespace>
        <oboInOwl:id>GAZ:00053554</oboInOwl:id>
        <rdfs:label>Emuruangogolak Volcano</rdfs:label>
    </owl:NamedIndividual>
    


    <!-- http://purl.obolibrary.org/obo/GAZ_00053555 -->

    <owl:NamedIndividual rdf:about="http://purl.obolibrary.org/obo/GAZ_00053555">
        <obo:RO_0001025 rdf:resource="http://purl.obolibrary.org/obo/GAZ_00000007"/>
        <obo:IAO_0000115>A trachytic shield volcano, the largest Quaternary volcano in the northern Gregory Rift, completely straddles the East African Rift. An impressive 5 x 8 km summit caldera with 300 m deep walls is thought to have formed about 63,000 years ago. Caldera formation is thought to have been incremental, related to eruption of the Kantenmening basaltic and trachytic lava flows. A series of summit-area lava benches formed by eruptions from circumferential fissures has produced a volcano morphologically similar to Galapagos Islands volcanoes. Northern, eastern, and southern flanks are cut by a prominent broad rift zone 10 km wide and 30 km long, dotted with numerous pyroclastic cones. Lava domes on the upper eastern flank formed during the late Pleistocene and early Holocene, until about 7 ka. Youthful parasitic cones abound on the caldera floor and on the northern and NE flanks; the youngest lava flows may be little more than a few hundred years old (Williams et al. 1984). Geothermal activity occurs within the caldera and on the upper eastern flanks.</obo:IAO_0000115>
        <oboInOwl:hasOBONamespace>GAZ</oboInOwl:hasOBONamespace>
        <oboInOwl:id>GAZ:00053555</oboInOwl:id>
        <rdfs:label>Silali Volcano</rdfs:label>
    </owl:NamedIndividual>
    


    <!-- http://purl.obolibrary.org/obo/GAZ_00053556 -->

    <owl:NamedIndividual rdf:about="http://purl.obolibrary.org/obo/GAZ_00053556">
        <obo:RO_0001025 rdf:resource="http://purl.obolibrary.org/obo/GAZ_00000007"/>
        <obo:IAO_0000115>A shield volcano in the Gregory Rift contains a small 1.5 km wide summit caldera. Eruption of large volumes of trachytic pyroclastic rocks around the end of the Pleistocene and the beginning of the Holocene formed a NW-trending ridge of pyroclastic cones across the summit region; collapse of this area formed the summit caldera and associated craters. A second large crater SE of the caldera is 0.5 x 1 km wide and contains a pumice cone. The summit caldera is narrowly breached on the north side, which has funneled post-caldera lava flows in this direction. The three youngest post-caldera pyroclastic cones on the NE flank may be only a few hundred years old. A series of viscous trachytic lava flows were erupted from vents on the volcano&apos;s lower flanks. Young fissure-fed basalts were also erupted to the south, between Paka and Korosi volcanoes. Surficial geothermal activity is widespread at Paka both within the summit caldera and on extensive portions of the northern flank.</obo:IAO_0000115>
        <oboInOwl:hasOBONamespace>GAZ</oboInOwl:hasOBONamespace>
        <oboInOwl:id>GAZ:00053556</oboInOwl:id>
        <rdfs:label>Paka Volcano</rdfs:label>
    </owl:NamedIndividual>
    


    <!-- http://purl.obolibrary.org/obo/GAZ_00053557 -->

    <owl:NamedIndividual rdf:about="http://purl.obolibrary.org/obo/GAZ_00053557">
        <obo:RO_0001025 rdf:resource="http://purl.obolibrary.org/obo/GAZ_00000007"/>
        <obo:IAO_0000115>A broad shield volcano west of Lake Bogoria that has been cut by spectacular grid faults along the west margin of the Gregory Rift. Geysers on the west margin of Lake Bogoria may be of tectonic origin.</obo:IAO_0000115>
        <oboInOwl:hasOBONamespace>GAZ</oboInOwl:hasOBONamespace>
        <oboInOwl:id>GAZ:00053557</oboInOwl:id>
        <rdfs:label>Bogoria Volcano</rdfs:label>
    </owl:NamedIndividual>
    


    <!-- http://purl.obolibrary.org/obo/GAZ_00053558 -->

    <owl:NamedIndividual rdf:about="http://purl.obolibrary.org/obo/GAZ_00053558">
        <obo:RO_0001025 rdf:resource="http://purl.obolibrary.org/obo/GAZ_00000007"/>
        <obo:IAO_0000115>A shield volcano that lies at the north end of Lake Baringo. Unlike other rift valley volcanoes, it does not contain a summit caldera. Lava domes on the northern flanks have fed trachytic lava flows. The major stage of Korosi volcanism spanned a period between 0.4 and 0.1 million years ago and included the eruption of voluminous fluid basaltic lava flows and pyroclastic cone formation along a NNE-trending fissure cutting across the axis of the shield volcano. This was followed by the eruption of trachytic lava domes and pumice/scoria cones. The youngest activity, consisting of fissure-fed basaltic lava flows on the lower northern flanks between Korosi and Paka, was probably coeval with the latest eruptions on Ol Kokwe to the south, which are only a few hundred to a few thousand years old (Dunkley et al. 1993). Fumaroles and hot steaming ground occur around the summit cones and NW flanks over an area of 30 sq km.</obo:IAO_0000115>
        <oboInOwl:hasOBONamespace>GAZ</oboInOwl:hasOBONamespace>
        <oboInOwl:id>GAZ:00053558</oboInOwl:id>
        <rdfs:label>Korosi Volcano</rdfs:label>
    </owl:NamedIndividual>
    


    <!-- http://purl.obolibrary.org/obo/GAZ_00053560 -->

    <owl:NamedIndividual rdf:about="http://purl.obolibrary.org/obo/GAZ_00053560">
        <obo:RO_0001025 rdf:resource="http://purl.obolibrary.org/obo/GAZ_00000007"/>
        <obo:IAO_0000115>A shield volcano that occupies the floor of the East African Rift. Construction of a 30 cu km shield volcano beginning about 200,000 years ago was followed by the eruption of two voluminous ash-flow tuffs, each preceded by major pumice falls.</obo:IAO_0000115>
        <oboInOwl:hasOBONamespace>GAZ</oboInOwl:hasOBONamespace>
        <oboInOwl:id>GAZ:00053560</oboInOwl:id>
        <rdfs:label>Menengai Volcano</rdfs:label>
    </owl:NamedIndividual>
    


    <!-- http://purl.obolibrary.org/obo/GAZ_00053565 -->

    <owl:NamedIndividual rdf:about="http://purl.obolibrary.org/obo/GAZ_00053565">
        <obo:RO_0001025 rdf:resource="http://purl.obolibrary.org/obo/GAZ_00000007"/>
        <obo:IAO_0000115>A volcanic field located between Lake Elmenteita and Eburru volcano, is an area of pyroclastic cones and lava flows of varying ages.</obo:IAO_0000115>
        <oboInOwl:hasOBONamespace>GAZ</oboInOwl:hasOBONamespace>
        <oboInOwl:id>GAZ:00053565</oboInOwl:id>
        <rdfs:label>Elmenteita Badlands</rdfs:label>
    </owl:NamedIndividual>
    


    <!-- http://purl.obolibrary.org/obo/GAZ_00053566 -->

    <owl:NamedIndividual rdf:about="http://purl.obolibrary.org/obo/GAZ_00053566">
        <obo:RO_0001025 rdf:resource="http://purl.obolibrary.org/obo/GAZ_00000007"/>
        <obo:IAO_0000115>A comple volcano that is elongated perpendicular to the Gregory Rift NW of Lake Naivasha. The 2856 m high, E-W-trending main edifice is eroded, but young partly vegetated rhyolitic domes occur on the east flank and are probably of Holocene age A prominent late-Pleistocene rhyolitic lava flow from a SE-flank vents extends almost to Lake Naivasha. Extensive fumarolic activity occurs at cinder cones and craters constructed along dominantly N-S-trending faults cutting the massif.</obo:IAO_0000115>
        <oboInOwl:hasOBONamespace>GAZ</oboInOwl:hasOBONamespace>
        <oboInOwl:id>GAZ:00053566</oboInOwl:id>
        <rdfs:label>Ol Doinyo Eburru Volcanic Complex</rdfs:label>
    </owl:NamedIndividual>
    


    <!-- http://purl.obolibrary.org/obo/GAZ_00053567 -->

    <owl:NamedIndividual rdf:about="http://purl.obolibrary.org/obo/GAZ_00053567">
        <obo:RO_0001025 rdf:resource="http://purl.obolibrary.org/obo/GAZ_00000007"/>
        <obo:IAO_0000115>A volcanic complex, located immediately south of Lake Naivasha and west of Longonot volcano, comprises up to 80 individual commenditic and other peralkaline rhyolitic centers. A thick, geochemically diverse basal complex is overlain by a dominantly silicic lava-dome and lava-flow complex active from about 20,000 years ago to the present. The youngest known eruption originated from the Ololbutot fissure on the SE side of the complex produced lava flows and a pumice flow and has a radiocarbon age of about 180 years. Fumarolic activity occurs at the Njorowa Gorge and at the Orengingnai and Olkaria (Orgaria) pumice cones.</obo:IAO_0000115>
        <oboInOwl:hasOBONamespace>GAZ</oboInOwl:hasOBONamespace>
        <oboInOwl:id>GAZ:00053567</oboInOwl:id>
        <rdfs:label>Olkaria Volcanic Complex</rdfs:label>
    </owl:NamedIndividual>
    


    <!-- http://purl.obolibrary.org/obo/GAZ_00053568 -->

    <owl:NamedIndividual rdf:about="http://purl.obolibrary.org/obo/GAZ_00053568">
        <obo:RO_0001025 rdf:resource="http://purl.obolibrary.org/obo/GAZ_00053569"/>
        <obo:IAO_0000115>A stratovolcano SE of Lake Naivasha in the Gregory Rift valley contains a 8 x 12 km caldera. Formation of the caldera accompanied large explosive eruptions about 21,000 years ago. A large central cone that was constructed within the caldera forms the 2776 m high summit of the volcano. The younger cone is truncated by a circular, 1.8 km wide crater. Post-caldera lavas are found on the caldera floor and the volcano&apos;s flanks, marking a late stage of effusive eruptions. A well-preserved satellitic cone is located on the NE flank.</obo:IAO_0000115>
        <oboInOwl:hasOBONamespace>GAZ</oboInOwl:hasOBONamespace>
        <oboInOwl:id>GAZ:00053568</oboInOwl:id>
        <rdfs:label>Mount Longonot</rdfs:label>
    </owl:NamedIndividual>
    


    <!-- http://purl.obolibrary.org/obo/GAZ_00053569 -->

    <owl:NamedIndividual rdf:about="http://purl.obolibrary.org/obo/GAZ_00053569">
        <obo:RO_0001025 rdf:resource="http://purl.obolibrary.org/obo/GAZ_00000007"/>
        <oboInOwl:hasOBONamespace>GAZ</oboInOwl:hasOBONamespace>
        <oboInOwl:id>GAZ:00053569</oboInOwl:id>
        <rdfs:label>Mount Longonot National Park</rdfs:label>
    </owl:NamedIndividual>
    


    <!-- http://purl.obolibrary.org/obo/GAZ_00053570 -->

    <owl:NamedIndividual rdf:about="http://purl.obolibrary.org/obo/GAZ_00053570">
        <obo:RO_0001025 rdf:resource="http://purl.obolibrary.org/obo/GAZ_00000007"/>
        <obo:IAO_0000115>A caldera of the Kenya rift, Suswa contains a prominent lava cone on the south side of its 8 x 12 km caldera. Suswa lies south of Longonot volcano and about 50 km WNW of the capital city of Nairobi. Construction of an early shield volcano was followed by eruption of voluminous Pleistocene pumice flows and lava flows that accompanied incremental formation of the caldera.</obo:IAO_0000115>
        <oboInOwl:hasOBONamespace>GAZ</oboInOwl:hasOBONamespace>
        <oboInOwl:id>GAZ:00053570</oboInOwl:id>
        <rdfs:label>Suswa Volcano</rdfs:label>
    </owl:NamedIndividual>
    


    <!-- http://purl.obolibrary.org/obo/GAZ_00053571 -->

    <owl:NamedIndividual rdf:about="http://purl.obolibrary.org/obo/GAZ_00053571">
        <obo:RO_0001025 rdf:resource="http://purl.obolibrary.org/obo/GAZ_00053570"/>
        <obo:IAO_0000115>A post-caldera lava cone.</obo:IAO_0000115>
        <oboInOwl:hasOBONamespace>GAZ</oboInOwl:hasOBONamespace>
        <oboInOwl:id>GAZ:00053571</oboInOwl:id>
        <rdfs:label>Ol Doinyo Onyoke</rdfs:label>
    </owl:NamedIndividual>
    


    <!-- http://purl.obolibrary.org/obo/GAZ_00053591 -->

    <owl:NamedIndividual rdf:about="http://purl.obolibrary.org/obo/GAZ_00053591">
        <obo:RO_0001025 rdf:resource="http://purl.obolibrary.org/obo/GAZ_00000007"/>
        <obo:IAO_0000115>A national park that protects Lake Nakuru, near Nakuru Town.</obo:IAO_0000115>
        <oboInOwl:hasOBONamespace>GAZ</oboInOwl:hasOBONamespace>
        <oboInOwl:id>GAZ:00053591</oboInOwl:id>
        <rdfs:label>Lake Nakuru National Park</rdfs:label>
    </owl:NamedIndividual>
    


    <!-- http://purl.obolibrary.org/obo/GAZ_00053598 -->

    <owl:NamedIndividual rdf:about="http://purl.obolibrary.org/obo/GAZ_00053598">
        <obo:RO_0001025 rdf:resource="http://purl.obolibrary.org/obo/GAZ_00051205"/>
        <obo:IAO_0000115>A stratovolcano that occupies an isolated location in the arid Danakil depression. It contains a large, central volcanotectonic depression that is open to the Zula Gulf and an isolated central cone. Jalua lies NW of basaltic lava flows of the Alid graben and south of the Zula Gulf.</obo:IAO_0000115>
        <oboInOwl:hasOBONamespace>GAZ</oboInOwl:hasOBONamespace>
        <oboInOwl:id>GAZ:00053598</oboInOwl:id>
        <rdfs:label>Jalua Volcano</rdfs:label>
    </owl:NamedIndividual>
    


    <!-- http://purl.obolibrary.org/obo/GAZ_00053599 -->

    <owl:NamedIndividual rdf:about="http://purl.obolibrary.org/obo/GAZ_00053599">
        <obo:RO_0001025 rdf:resource="http://purl.obolibrary.org/obo/GAZ_00051205"/>
        <obo:IAO_0000115>An isolated, dissected stratovolcano in the central Danakil depression. The volcano is elongated in an E-W direction perpendicular to the orientation of the Alid graben. Alid consists of a structural dome of uplifted sedimentary rocks, capped by basaltic-to-rhyolitic lava flows, that rises 700 m above the graben floor.</obo:IAO_0000115>
        <oboInOwl:hasOBONamespace>GAZ</oboInOwl:hasOBONamespace>
        <oboInOwl:id>GAZ:00053599</oboInOwl:id>
        <rdfs:label>Alid Volcano</rdfs:label>
    </owl:NamedIndividual>
    


    <!-- http://purl.obolibrary.org/obo/GAZ_00053600 -->

    <owl:NamedIndividual rdf:about="http://purl.obolibrary.org/obo/GAZ_00053600">
        <obo:RO_0001025 rdf:resource="http://purl.obolibrary.org/obo/GAZ_00053602"/>
        <obo:IAO_0000115>Numerous phreatic explosion craters dot the Salt Plain NNE of the Erta Ale Range in one of the lowest areas of the desolate Danakil depression. These craters mark Earth&apos;s lowest known subaerial volcanic vents.</obo:IAO_0000115>
        <oboInOwl:hasOBONamespace>GAZ</oboInOwl:hasOBONamespace>
        <oboInOwl:id>GAZ:00053600</oboInOwl:id>
        <rdfs:label>Dallol Volcano</rdfs:label>
    </owl:NamedIndividual>
    


    <!-- http://purl.obolibrary.org/obo/GAZ_00053601 -->

    <owl:NamedIndividual rdf:about="http://purl.obolibrary.org/obo/GAZ_00053601">
        <obo:RO_0001025 rdf:resource="http://purl.obolibrary.org/obo/GAZ_00053602"/>
        <obo:IAO_0000115>A prominent stratovolcano at the northern end of the Erta Ale Range. It is formed of interstratified lava flows and hyaloclastites. Fumarolic activity is continuing, and a small lake filled by boiling mud occupies the crater.</obo:IAO_0000115>
        <oboInOwl:hasOBONamespace>GAZ</oboInOwl:hasOBONamespace>
        <oboInOwl:id>GAZ:00053601</oboInOwl:id>
        <rdfs:label>Gada Ale Volcano</rdfs:label>
    </owl:NamedIndividual>
    


    <!-- http://purl.obolibrary.org/obo/GAZ_00053602 -->

    <owl:NamedIndividual rdf:about="http://purl.obolibrary.org/obo/GAZ_00053602">
        <obo:RO_0001025 rdf:resource="http://purl.obolibrary.org/obo/GAZ_00000779"/>
        <obo:RO_0001025 rdf:resource="http://purl.obolibrary.org/obo/GAZ_00051205"/>
        <obo:IAO_0000115>An axial volcanic chain of the Afar Region, Ethiopia. It consists mostly of shield volcanoes.</obo:IAO_0000115>
        <oboInOwl:hasOBONamespace>GAZ</oboInOwl:hasOBONamespace>
        <oboInOwl:id>GAZ:00053602</oboInOwl:id>
        <rdfs:label>Erta Ale Range</rdfs:label>
    </owl:NamedIndividual>
    


    <!-- http://purl.obolibrary.org/obo/GAZ_00053603 -->

    <owl:NamedIndividual rdf:about="http://purl.obolibrary.org/obo/GAZ_00053603">
        <obo:RO_0001025 rdf:resource="http://purl.obolibrary.org/obo/GAZ_00053602"/>
        <obo:IAO_0000115>An active shield volcano located in the Afar Region of northeastern Ethiopia. It is the most active volcano in Ethiopia. The broad, 50 km wide volcano rises more than 600 m from below sea level in the barren Danakil depression.</obo:IAO_0000115>
        <oboInOwl:hasOBONamespace>GAZ</oboInOwl:hasOBONamespace>
        <oboInOwl:id>GAZ:00053603</oboInOwl:id>
        <rdfs:label>Erta Ale Volcano</rdfs:label>
    </owl:NamedIndividual>
    


    <!-- http://purl.obolibrary.org/obo/GAZ_00053604 -->

    <owl:NamedIndividual rdf:about="http://purl.obolibrary.org/obo/GAZ_00053604">
        <obo:RO_0001025 rdf:resource="http://purl.obolibrary.org/obo/GAZ_00053602"/>
        <obo:IAO_0000115>An elongated, 1031 m high stratovolcano located SW of Erta Ale volcano. It is the highest of the Erta Ale Range volcanoes and is located west of the axis of the range. In contrast to other volcanoes of the Erta Ale Range, Ale Bagu is mantled by basaltic pyroclastic rocks. Summit craters are elongated along a NNW-SSE trend. The main crater is a steep-walled, 750 x 450 m depression occupied by a steep-sided lava cone that has fed trachytic lava flows over the crater floor.</obo:IAO_0000115>
        <oboInOwl:hasOBONamespace>GAZ</oboInOwl:hasOBONamespace>
        <oboInOwl:id>GAZ:00053604</oboInOwl:id>
        <rdfs:label>Ale Bagu Volcano</rdfs:label>
    </owl:NamedIndividual>
    


    <!-- http://purl.obolibrary.org/obo/GAZ_00053605 -->

    <owl:NamedIndividual rdf:about="http://purl.obolibrary.org/obo/GAZ_00053605">
        <obo:RO_0001025 rdf:resource="http://purl.obolibrary.org/obo/GAZ_00053602"/>
        <obo:RO_0001025 rdf:resource="http://purl.obolibrary.org/obo/GAZ_00123434"/>
        <obo:IAO_0000115>A small, but steep-sided conical stratovolcano that rises 300 m above surrounding lava fields SE of Alu volcano. This morphology, unusual for the Erta Ale Range volcanoes, results from the extrusion of viscous, silicic lava flows with primary slopes up to about 35 degrees. These silicic flows extend primarily to the east; on the west they are blocked by walls of a horst structure along the crest of the Erta Ale range.</obo:IAO_0000115>
        <oboInOwl:hasOBONamespace>GAZ</oboInOwl:hasOBONamespace>
        <oboInOwl:id>GAZ:00053605</oboInOwl:id>
        <rdfs:label>Dalaffilla Volcano</rdfs:label>
    </owl:NamedIndividual>
    


    <!-- http://purl.obolibrary.org/obo/GAZ_00053606 -->

    <owl:NamedIndividual rdf:about="http://purl.obolibrary.org/obo/GAZ_00053606">
        <obo:RO_0001025 rdf:resource="http://purl.obolibrary.org/obo/GAZ_00053602"/>
        <obo:IAO_0000115>A system of volcanic fissures, located in Ethiopia. The fissures have produced silicic lava flows, and other fissures south of the volcano have formed huge youthful basaltic lava flows, which enlarge to the north as far as Lake Bakili. There is major fumarolic motion, which are located on frequent corresponding faults, some of which gave a lift up to 100 m.</obo:IAO_0000115>
        <oboInOwl:hasOBONamespace>GAZ</oboInOwl:hasOBONamespace>
        <oboInOwl:id>GAZ:00053606</oboInOwl:id>
        <rdfs:label>Alu Fissure Vents</rdfs:label>
    </owl:NamedIndividual>
    


    <!-- http://purl.obolibrary.org/obo/GAZ_00053607 -->

    <owl:NamedIndividual rdf:about="http://purl.obolibrary.org/obo/GAZ_00053607">
        <obo:RO_0001025 rdf:resource="http://purl.obolibrary.org/obo/GAZ_00053602"/>
        <obo:IAO_0000115>A complex stratovolcano located near the center of the Erta Ale Range. The earliest activity formed submarine lava flows partially covered by Quaternary reef deposits. An embryonic shield volcano is located on the SW side of the complex and is cut by curvilinear faults; youthful chains of spatter cones follow this same curvilinear pattern and form concentric semi-circles. The 668 m high summit of the Borale Ale complex is located on the NE side of the massif and consists of a silicic stratovolcano that is the largest of the Erte Ale Range. It has produced steep-sided viscous lava flows that have traveled up to 5 km from the volcano. Strong fumarolic activity occurs within a 300-m-wide summit crater.</obo:IAO_0000115>
        <oboInOwl:hasOBONamespace>GAZ</oboInOwl:hasOBONamespace>
        <oboInOwl:id>GAZ:00053607</oboInOwl:id>
        <rdfs:label>Borale Ale Volcano</rdfs:label>
    </owl:NamedIndividual>
    


    <!-- http://purl.obolibrary.org/obo/GAZ_00053608 -->

    <owl:NamedIndividual rdf:about="http://purl.obolibrary.org/obo/GAZ_00053608">
        <obo:RO_0001025 rdf:resource="http://purl.obolibrary.org/obo/GAZ_00053602"/>
        <obo:IAO_0000115>A shield volcano where tectonism has created a graben at the 521 m high summit. A symmetrical scoria cone with a 200-m-wide crater displaying fumarolic activity occupies the center of the graben. An older shield volcano is covered on the north by recent fissure-fed lava flows. Lava flows from the axial portion of a fissure system extending to the south have reached the floor of the Giulietti Plain south of the Erta Ale Range. The open fissures extend for more than 10 km and are lined with dozens of small spatter cones and pit craters.</obo:IAO_0000115>
        <oboInOwl:hasOBONamespace>GAZ</oboInOwl:hasOBONamespace>
        <oboInOwl:id>GAZ:00053608</oboInOwl:id>
        <rdfs:label>Hayli Gubbi Volcano</rdfs:label>
    </owl:NamedIndividual>
    


    <!-- http://purl.obolibrary.org/obo/GAZ_00053609 -->

    <owl:NamedIndividual rdf:about="http://purl.obolibrary.org/obo/GAZ_00053609">
        <obo:RO_0001025 rdf:resource="http://purl.obolibrary.org/obo/GAZ_00051205"/>
        <obo:IAO_0000115>A stratovolcano located east of the Erta Ale Range and south of the crystalline basement rocks of the Danakil Alps. It is a large volcanic massif that rises to 1625 m above the western shore of the Red Sea. About 20 small cinder cones are located at the summit, and extensive basaltic lava fields to the north and NE, known as the Edd lava field, cover an area of 2700 km2 and reach the Red Sea coast.</obo:IAO_0000115>
        <oboInOwl:hasOBONamespace>GAZ</oboInOwl:hasOBONamespace>
        <oboInOwl:id>GAZ:00053609</oboInOwl:id>
        <rdfs:label>Dubbi Volcano</rdfs:label>
    </owl:NamedIndividual>
    


    <!-- http://purl.obolibrary.org/obo/GAZ_00053610 -->

    <owl:NamedIndividual rdf:about="http://purl.obolibrary.org/obo/GAZ_00053610">
        <obo:RO_0001025 rdf:resource="http://purl.obolibrary.org/obo/GAZ_00051205"/>
        <obo:IAO_0000115>A stratovolcano in the Danakil depression of northern Ethiopia and Eritrea. Located at the SE end of the Danakil Alps, Nabro lies in the Danakil horst. Nabro is the most prominent and NE-most of three volcanoes with large summit calderas aligned in a NE-SW direction SW of Dubbi volcano. These three volcanoes, along with Sork Ale volcano, collectively comprise the Bidu volcanic complex. The complex Nabro stratovolcano is truncated by nested calderas, 8 and 5 km in diameter. The larger caldera is widely breached to the SW. Nabro was constructed primarily of trachytic lava flows and pyroclastics. Post-caldera rhyolitic obsidian domes and basaltic lava flows were erupted inside the caldera and on its flanks.</obo:IAO_0000115>
        <oboInOwl:hasOBONamespace>GAZ</oboInOwl:hasOBONamespace>
        <oboInOwl:id>GAZ:00053610</oboInOwl:id>
        <rdfs:label>Nabro Volcano</rdfs:label>
    </owl:NamedIndividual>
    


    <!-- http://purl.obolibrary.org/obo/GAZ_00053611 -->

    <owl:NamedIndividual rdf:about="http://purl.obolibrary.org/obo/GAZ_00053611">
        <obo:RO_0001025 rdf:resource="http://purl.obolibrary.org/obo/GAZ_00000784"/>
        <oboInOwl:hasOBONamespace>GAZ</oboInOwl:hasOBONamespace>
        <oboInOwl:id>GAZ:00053611</oboInOwl:id>
        <rdfs:label>Bidu Volcanic Complex</rdfs:label>
    </owl:NamedIndividual>
    


    <!-- http://purl.obolibrary.org/obo/GAZ_00053612 -->

    <owl:NamedIndividual rdf:about="http://purl.obolibrary.org/obo/GAZ_00053612">
        <obo:RO_0001025 rdf:resource="http://purl.obolibrary.org/obo/GAZ_00053611"/>
        <obo:IAO_0000115>A silicic stratovolcano located in the Danakil horst SE of Mallahle volcano. Sork Ale was constructed perpendicular to the NE-SW orientation of three larger stratovolcanoes of the Nabro volcanic range at the southern end of the Danakil Alps. A small, roughly 1 km wide, 300-m-deep steep-walled caldera is found at the summit of the 1611 m high volcano. Basaltic lava flows are prominent on the eastern side of the volcano, and satellite vents are located on the SE flank.</obo:IAO_0000115>
        <oboInOwl:hasOBONamespace>GAZ</oboInOwl:hasOBONamespace>
        <oboInOwl:id>GAZ:00053612</oboInOwl:id>
        <rdfs:label>Sork&apos;Ale Volcano</rdfs:label>
    </owl:NamedIndividual>
    


    <!-- http://purl.obolibrary.org/obo/GAZ_00053613 -->

    <owl:NamedIndividual rdf:about="http://purl.obolibrary.org/obo/GAZ_00053613">
        <obo:RO_0001025 rdf:resource="http://purl.obolibrary.org/obo/GAZ_00053611"/>
        <oboInOwl:hasOBONamespace>GAZ</oboInOwl:hasOBONamespace>
        <oboInOwl:id>GAZ:00053613</oboInOwl:id>
        <rdfs:label>Bara Ale Volcano</rdfs:label>
    </owl:NamedIndividual>
    


    <!-- http://purl.obolibrary.org/obo/GAZ_00053614 -->

    <owl:NamedIndividual rdf:about="http://purl.obolibrary.org/obo/GAZ_00053614">
        <obo:RO_0001025 rdf:resource="http://purl.obolibrary.org/obo/GAZ_00053611"/>
        <obo:IAO_0000115>A stratovolcano in the Danakil horst SW of Dubbi volcano, and lies SSW of Nabro volcano. These two volcanoes, along with Bara Ale and Sork&apos;Ale, form the Bidu volcanic complex. The complex Mallahle stratovolcano is truncated by a steep-walled 6 km wide caldera. Mallahle is formed of rhyolitic lava flows and pyroclastics. Basaltic lava flows blanket the slopes of the volcano.</obo:IAO_0000115>
        <oboInOwl:hasOBONamespace>GAZ</oboInOwl:hasOBONamespace>
        <oboInOwl:id>GAZ:00053614</oboInOwl:id>
        <rdfs:label>Mallahle Volcano</rdfs:label>
    </owl:NamedIndividual>
    


    <!-- http://purl.obolibrary.org/obo/GAZ_00053615 -->

    <owl:NamedIndividual rdf:about="http://purl.obolibrary.org/obo/GAZ_00053615">
        <obo:RO_0001025 rdf:resource="http://purl.obolibrary.org/obo/GAZ_00000567"/>
        <obo:IAO_0000115>A shield volcano constructed along a NE-SW-trending line in the Danakil horst. A large 12 km wide caldera truncates the summit of the volcano. Basaltic lava flows blanket the flanks of Asavyo, which merge into the Mogorros plains to the south.</obo:IAO_0000115>
        <oboInOwl:hasOBONamespace>GAZ</oboInOwl:hasOBONamespace>
        <oboInOwl:id>GAZ:00053615</oboInOwl:id>
        <rdfs:label>Asavyo Volcano</rdfs:label>
    </owl:NamedIndividual>
    


    <!-- http://purl.obolibrary.org/obo/GAZ_00053616 -->

    <owl:NamedIndividual rdf:about="http://purl.obolibrary.org/obo/GAZ_00053616">
        <obo:RO_0001025 rdf:resource="http://purl.obolibrary.org/obo/GAZ_00053617"/>
        <obo:IAO_0000115>A low, 523 m high shield volcano in the southern Tat Ali Range, east of Afdera volcano. A 300-m-deep, 2.5 x 3.5 km wide caldera is found at the summit of the volcano, whose flanks are cut by numerous N-S-trending faults.</obo:IAO_0000115>
        <oboInOwl:hasOBONamespace>GAZ</oboInOwl:hasOBONamespace>
        <oboInOwl:id>GAZ:00053616</oboInOwl:id>
        <rdfs:label>Mat Ala Volcano</rdfs:label>
    </owl:NamedIndividual>
    


    <!-- http://purl.obolibrary.org/obo/GAZ_00053617 -->

    <owl:NamedIndividual rdf:about="http://purl.obolibrary.org/obo/GAZ_00053617">
        <obo:RO_0001025 rdf:resource="http://purl.obolibrary.org/obo/GAZ_00000779"/>
        <obo:IAO_0000115>A mountain range to the E of Lake Afrera.</obo:IAO_0000115>
        <oboInOwl:hasOBONamespace>GAZ</oboInOwl:hasOBONamespace>
        <oboInOwl:id>GAZ:00053617</oboInOwl:id>
        <rdfs:label>Tat Ali Range</rdfs:label>
    </owl:NamedIndividual>
    


    <!-- http://purl.obolibrary.org/obo/GAZ_00053618 -->

    <owl:NamedIndividual rdf:about="http://purl.obolibrary.org/obo/GAZ_00053618">
        <obo:RO_0001025 rdf:resource="http://purl.obolibrary.org/obo/GAZ_00053617"/>
        <obo:IAO_0000115>A low shield volcano has an elongated summit depression and has produced a variety of rock types, ranging from basalts to pantellerites. NNW-SSE-trending fissures cutting the volcano have fed basaltic lava flows; those NE of Lake Afrera are of prehistorical age. Late-stage volcanism produced youthful basaltic lava flows on the floor of the summit depression, which is also the site of prominent fumarolic activity.</obo:IAO_0000115>
        <oboInOwl:hasOBONamespace>GAZ</oboInOwl:hasOBONamespace>
        <oboInOwl:id>GAZ:00053618</oboInOwl:id>
        <rdfs:label>Tat Ali Volcano</rdfs:label>
    </owl:NamedIndividual>
    


    <!-- http://purl.obolibrary.org/obo/GAZ_00053619 -->

    <owl:NamedIndividual rdf:about="http://purl.obolibrary.org/obo/GAZ_00053619">
        <obo:RO_0001025 rdf:resource="http://purl.obolibrary.org/obo/GAZ_00031086"/>
        <obo:RO_0001025 rdf:resource="http://purl.obolibrary.org/obo/GAZ_00051205"/>
        <obo:IAO_0000115>A saline lake in northern Ethiopia. Located in the Administrative Zone 2, it is one of the lakes of the Afar Depression.</obo:IAO_0000115>
        <oboInOwl:hasOBONamespace>GAZ</oboInOwl:hasOBONamespace>
        <oboInOwl:id>GAZ:00053619</oboInOwl:id>
        <rdfs:label>Lake Afrera</rdfs:label>
    </owl:NamedIndividual>
    


    <!-- http://purl.obolibrary.org/obo/GAZ_00053620 -->

    <owl:NamedIndividual rdf:about="http://purl.obolibrary.org/obo/GAZ_00053620">
        <obo:RO_0001025 rdf:resource="http://purl.obolibrary.org/obo/GAZ_00031086"/>
        <obo:RO_0001025 rdf:resource="http://purl.obolibrary.org/obo/GAZ_00053632"/>
        <obo:IAO_0000115>A stratovolcano that rises above the eastern shore of Lake Afrera, also known as Lake Giulietti. The upper part of the 812 m high conical volcano consists of trachytic lava flows overlying older basaltic flows. Young pantelleritic obsidian domes south of the volcano are the probable source of rounded pumice fragments found around Lake Afrera.</obo:IAO_0000115>
        <oboInOwl:hasOBONamespace>GAZ</oboInOwl:hasOBONamespace>
        <oboInOwl:id>GAZ:00053620</oboInOwl:id>
        <rdfs:label>Borawli Volcano</rdfs:label>
    </owl:NamedIndividual>
    


    <!-- http://purl.obolibrary.org/obo/GAZ_00053621 -->

    <owl:NamedIndividual rdf:about="http://purl.obolibrary.org/obo/GAZ_00053621">
        <obo:RO_0001025 rdf:resource="http://purl.obolibrary.org/obo/GAZ_00000779"/>
        <obo:IAO_0000115>An isolated rhyolitic stratovolcano located between the Erta Ale, Tat Ali, and Alayta ranges. It lies at the intersection of three fault systems. Young rhyolitic lava domes are aligned N-S at its southern foot. Only a few late-stage satellitic cones are of basaltic composition.</obo:IAO_0000115>
        <oboInOwl:hasOBONamespace>GAZ</oboInOwl:hasOBONamespace>
        <oboInOwl:id>GAZ:00053621</oboInOwl:id>
        <rdfs:label>Afdera Volcano</rdfs:label>
    </owl:NamedIndividual>
    


    <!-- http://purl.obolibrary.org/obo/GAZ_00053622 -->

    <owl:NamedIndividual rdf:about="http://purl.obolibrary.org/obo/GAZ_00053622">
        <obo:RO_0001025 rdf:resource="http://purl.obolibrary.org/obo/GAZ_00000779"/>
        <obo:RO_0001025 rdf:resource="http://purl.obolibrary.org/obo/GAZ_00051205"/>
        <obo:IAO_0000115>An 1815 m high stratovolcano located well to the west of the Danakil depression at the foot of the regional Ethiopian scarp. The volcano is situated between two large horsts of uplifted basement blocks. A large trachytic and rhyolitic stratovolcano at the center of the Ma Alalta complex contains nested oval-shaped summit calderas, 8 x 5 km and 5 x 2.5 km wide. Ignimbrite deposits, perhaps associated with formation of the larger caldera, extend beyond the volcano primarily to the NE and SE. Young basaltic lava flows were erupted on the NW, SE, and eastern flanks of the volcano. Recent silicic activity has produced pantelleritic obsidian domes and lava flows on the volcano&apos;s southern flank. Fumarolic activity continues at one of the domes.</obo:IAO_0000115>
        <oboInOwl:hasOBONamespace>GAZ</oboInOwl:hasOBONamespace>
        <oboInOwl:id>GAZ:00053622</oboInOwl:id>
        <rdfs:label>Ma Alalta Volcano</rdfs:label>
    </owl:NamedIndividual>
    


    <!-- http://purl.obolibrary.org/obo/GAZ_00053623 -->

    <owl:NamedIndividual rdf:about="http://purl.obolibrary.org/obo/GAZ_00053623">
        <obo:RO_0001025 rdf:resource="http://purl.obolibrary.org/obo/GAZ_00000779"/>
        <obo:RO_0001025 rdf:resource="http://purl.obolibrary.org/obo/GAZ_00051205"/>
        <obo:IAO_0000115>A shield volcano covers an area of 2700 km2 in the western Danakil depression SW of Lake Afrera. A series of very recent craters is aligned along the NNW-trending axis of the basaltic-to-trachytic shield. The Alayta lava field, covered by very fresh lava flows, was erupted from N-S-trending fissures along the east side of the shield volcano and laps up against the western flank of Afdera volcano.</obo:IAO_0000115>
        <oboInOwl:hasOBONamespace>GAZ</oboInOwl:hasOBONamespace>
        <oboInOwl:id>GAZ:00053623</oboInOwl:id>
        <rdfs:label>Alayta Volcano</rdfs:label>
    </owl:NamedIndividual>
    


    <!-- http://purl.obolibrary.org/obo/GAZ_00053624 -->

    <owl:NamedIndividual rdf:about="http://purl.obolibrary.org/obo/GAZ_00053624">
        <obo:RO_0001025 rdf:resource="http://purl.obolibrary.org/obo/GAZ_00051205"/>
        <obo:RO_0001025 rdf:resource="http://purl.obolibrary.org/obo/GAZ_00123435"/>
        <obo:IAO_0000115>A Holocene stratovolcanic massif forming an axial range of the Afar depression SSW of the Alayta massif. Pantelleritic obsidian flows, lava domes, and pumice cones form the summit and upper flanks of the volcano, which rises above the Teru Plain and was built over a base of basaltic-to-trachytic lava flows of a shield volcano. Late-stage basaltic fissure eruptions occurred at the NW base of the volcano. Abundant fumaroles are located along the crest of the volcano and extend NE towards Alayta volcano.</obo:IAO_0000115>
        <oboInOwl:hasOBONamespace>GAZ</oboInOwl:hasOBONamespace>
        <oboInOwl:id>GAZ:00053624</oboInOwl:id>
        <rdfs:label>Dabbahu Volcano</rdfs:label>
    </owl:NamedIndividual>
    


    <!-- http://purl.obolibrary.org/obo/GAZ_00053625 -->

    <owl:NamedIndividual rdf:about="http://purl.obolibrary.org/obo/GAZ_00053625">
        <obo:RO_0001025 rdf:resource="http://purl.obolibrary.org/obo/GAZ_00000779"/>
        <obo:RO_0001025 rdf:resource="http://purl.obolibrary.org/obo/GAZ_00051205"/>
        <obo:IAO_0000115>A shield volcano that was constructed along an offshoot of the Ethiopian escarpment, SW of the Teru plain. In contrast to structural trends in other parts of Afar, Dabbayra consists of a basaltic shield volcano elongated in an ENE-WSW direction. The only silicic volcanic rocks are a NNW-trending line of lava domes and lava flows near the crest of the 1302 m high volcano.</obo:IAO_0000115>
        <oboInOwl:hasOBONamespace>GAZ</oboInOwl:hasOBONamespace>
        <oboInOwl:id>GAZ:00053625</oboInOwl:id>
        <rdfs:label>Dabbayra Volcano</rdfs:label>
    </owl:NamedIndividual>
    


    <!-- http://purl.obolibrary.org/obo/GAZ_00053626 -->

    <owl:NamedIndividual rdf:about="http://purl.obolibrary.org/obo/GAZ_00053626">
        <obo:RO_0001025 rdf:resource="http://purl.obolibrary.org/obo/GAZ_00000779"/>
        <obo:RO_0001025 rdf:resource="http://purl.obolibrary.org/obo/GAZ_00051205"/>
        <obo:IAO_0000115>A complex of shield volcanoes located in the Kalo plain, SSE of Dabbahu volcano. The massive complex is 105 km long and 20-30 km wide, and represents an uplifted segment of a mid-ocean ridge spreading center. A small basaltic shield volcano is located at the northern end of the complex, south of which is an area of abundant fissure-fed lava flows. Two basaltic shield volcanoes, the largest of which is Unda Hararo, occupy the center of the complex. The dominant part of the complex lies to the south, where the Gumatmali-Gablaytu fissure system is located. Voluminous fluid lava flows issued from these NNW-trending fissures, and solidified lava lakes occupy two large craters. The small Gablaytu shield volcano forms the SE-most end of the Manda Hararo complex. Lava flows from Gablaytu and from Manda overlie 8000-year-old sediments. Hot springs and fumaroles occur around Daorre lake.</obo:IAO_0000115>
        <oboInOwl:hasOBONamespace>GAZ</oboInOwl:hasOBONamespace>
        <oboInOwl:id>GAZ:00053626</oboInOwl:id>
        <rdfs:label>Manda Hararo Volcanic Complex</rdfs:label>
    </owl:NamedIndividual>
    


    <!-- http://purl.obolibrary.org/obo/GAZ_00053627 -->

    <owl:NamedIndividual rdf:about="http://purl.obolibrary.org/obo/GAZ_00053627">
        <obo:RO_0001025 rdf:resource="http://purl.obolibrary.org/obo/GAZ_00053626"/>
        <obo:IAO_0000115>A shield volcano.</obo:IAO_0000115>
        <oboInOwl:hasOBONamespace>GAZ</oboInOwl:hasOBONamespace>
        <oboInOwl:id>GAZ:00053627</oboInOwl:id>
        <rdfs:label>Gablaytu Volcano</rdfs:label>
    </owl:NamedIndividual>
    


    <!-- http://purl.obolibrary.org/obo/GAZ_00053628 -->

    <owl:NamedIndividual rdf:about="http://purl.obolibrary.org/obo/GAZ_00053628">
        <obo:RO_0001025 rdf:resource="http://purl.obolibrary.org/obo/GAZ_00053626"/>
        <obo:IAO_0000115>A fissure system.</obo:IAO_0000115>
        <oboInOwl:hasOBONamespace>GAZ</oboInOwl:hasOBONamespace>
        <oboInOwl:id>GAZ:00053628</oboInOwl:id>
        <rdfs:label>Gumatmali-Gablaytu Fissure System</rdfs:label>
    </owl:NamedIndividual>
    


    <!-- http://purl.obolibrary.org/obo/GAZ_00053629 -->

    <owl:NamedIndividual rdf:about="http://purl.obolibrary.org/obo/GAZ_00053629">
        <obo:RO_0001025 rdf:resource="http://purl.obolibrary.org/obo/GAZ_00053626"/>
        <obo:IAO_0000115>A basaltic shield volcano.</obo:IAO_0000115>
        <oboInOwl:hasOBONamespace>GAZ</oboInOwl:hasOBONamespace>
        <oboInOwl:id>GAZ:00053629</oboInOwl:id>
        <rdfs:label>Unda Hararo Volcano</rdfs:label>
    </owl:NamedIndividual>
    


    <!-- http://purl.obolibrary.org/obo/GAZ_00053630 -->

    <owl:NamedIndividual rdf:about="http://purl.obolibrary.org/obo/GAZ_00053630">
        <obo:RO_0001025 rdf:resource="http://purl.obolibrary.org/obo/GAZ_00000779"/>
        <obo:RO_0001025 rdf:resource="http://purl.obolibrary.org/obo/GAZ_00051205"/>
        <obo:IAO_0000115>A small 930 m high alkali rhyolitic stratovolcano located in the western Afar near the Ethiopian escarpment, NE of Dessye.</obo:IAO_0000115>
        <oboInOwl:hasOBONamespace>GAZ</oboInOwl:hasOBONamespace>
        <oboInOwl:id>GAZ:00053630</oboInOwl:id>
        <rdfs:label>Groppo Volcano</rdfs:label>
    </owl:NamedIndividual>
    


    <!-- http://purl.obolibrary.org/obo/GAZ_00053631 -->

    <owl:NamedIndividual rdf:about="http://purl.obolibrary.org/obo/GAZ_00053631">
        <obo:RO_0001025 rdf:resource="http://purl.obolibrary.org/obo/GAZ_00000779"/>
        <obo:RO_0001025 rdf:resource="http://purl.obolibrary.org/obo/GAZ_00051205"/>
        <obo:IAO_0000115>A shield volcano that lies in the Saha Plain, SE of the Manda Hararo complex in the South Danakil region. Wind-blown sand fills the summit crater of the young basaltic volcano. Initial subaqueous activity occurred along NNW-trending fissures. Fumarolic activity observed in the 1930s was not seen during field work in the 1970s.</obo:IAO_0000115>
        <oboInOwl:hasOBONamespace>GAZ</oboInOwl:hasOBONamespace>
        <oboInOwl:id>GAZ:00053631</oboInOwl:id>
        <rdfs:label>Kurub Volcano</rdfs:label>
    </owl:NamedIndividual>
    


    <!-- http://purl.obolibrary.org/obo/GAZ_00053632 -->

    <owl:NamedIndividual rdf:about="http://purl.obolibrary.org/obo/GAZ_00053632">
        <obo:RO_0001025 rdf:resource="http://purl.obolibrary.org/obo/GAZ_00051205"/>
        <obo:RO_0001025 rdf:resource="http://purl.obolibrary.org/obo/GAZ_00053617"/>
        <obo:IAO_0000115>A group of rhyolitic lava domes on the floor of the southern Kali plain, north of Aysa&apos;iyta.</obo:IAO_0000115>
        <oboInOwl:hasOBONamespace>GAZ</oboInOwl:hasOBONamespace>
        <oboInOwl:id>GAZ:00053632</oboInOwl:id>
        <rdfs:label>Borawli Volcanic Complex</rdfs:label>
    </owl:NamedIndividual>
    


    <!-- http://purl.obolibrary.org/obo/GAZ_00053633 -->

    <owl:NamedIndividual rdf:about="http://purl.obolibrary.org/obo/GAZ_00053633">
        <obo:RO_0001025 rdf:resource="http://purl.obolibrary.org/obo/GAZ_00000567"/>
        <obo:IAO_0000115>A series of NW-trending fissure vents and pyroclastic cones along the Ethiopia-Djibouti border. The elongated complex represents an uplifted mid-ocean ridge spreading center now exposed above sea level. An elongated dome of basement rocks is cut by two axial rifts, the northern of which was active during historical time. Basaltic cinder cones along marginal faults of the rift have produced lava flows that traveled down the flanks of the structural dome, producing a shield-like morphology.</obo:IAO_0000115>
        <oboInOwl:hasOBONamespace>GAZ</oboInOwl:hasOBONamespace>
        <oboInOwl:id>GAZ:00053633</oboInOwl:id>
        <rdfs:label>Manda-Inakir</rdfs:label>
    </owl:NamedIndividual>
    


    <!-- http://purl.obolibrary.org/obo/GAZ_00053634 -->

    <owl:NamedIndividual rdf:about="http://purl.obolibrary.org/obo/GAZ_00053634">
        <obo:RO_0001025 rdf:resource="http://purl.obolibrary.org/obo/GAZ_00053633"/>
        <obo:IAO_0000115>A cinder cone.</obo:IAO_0000115>
        <oboInOwl:hasOBONamespace>GAZ</oboInOwl:hasOBONamespace>
        <oboInOwl:id>GAZ:00053634</oboInOwl:id>
        <rdfs:label>Kammourta</rdfs:label>
    </owl:NamedIndividual>
    


    <!-- http://purl.obolibrary.org/obo/GAZ_00053635 -->

    <owl:NamedIndividual rdf:about="http://purl.obolibrary.org/obo/GAZ_00053635">
        <rdf:type rdf:resource="http://purl.obolibrary.org/obo/ENVO_00000354"/>
        <obo:RO_0001025 rdf:resource="http://purl.obolibrary.org/obo/GAZ_00000567"/>
        <obo:IAO_0000115>A volcanic complex that is a large Holocene stratovolcano constructed along the border between Ethiopia, Eritrea, and Djibouti. The 2028 m high trachytic-to-rhyolitic volcano is the most prominent topographic feature in this area and towers above its neighbor to the SW, Manda Inakir. Rhyolitic lava domes and lava flows are found in the summit region, which is truncated by a caldera.</obo:IAO_0000115>
        <oboInOwl:hasOBONamespace>GAZ</oboInOwl:hasOBONamespace>
        <oboInOwl:id>GAZ:00053635</oboInOwl:id>
        <rdfs:label>Mousa Alli Volcanic Complex</rdfs:label>
    </owl:NamedIndividual>
    


    <!-- http://purl.obolibrary.org/obo/GAZ_00053640 -->

    <owl:NamedIndividual rdf:about="http://purl.obolibrary.org/obo/GAZ_00053640">
        <obo:RO_0001025 rdf:resource="http://purl.obolibrary.org/obo/GAZ_00000567"/>
        <obo:IAO_0000115>A fumarole field immediately north of Lake Abbe. The fumaroles are located in a 7-m-deep funnel about 300 m above the surface of Lake Abbe and about 1 km NE of its shore; they are visible and audible from a distance.</obo:IAO_0000115>
        <oboInOwl:hasOBONamespace>GAZ</oboInOwl:hasOBONamespace>
        <oboInOwl:id>GAZ:00053640</oboInOwl:id>
        <rdfs:label>Boina Fumurole Field</rdfs:label>
    </owl:NamedIndividual>
    


    <!-- http://purl.obolibrary.org/obo/GAZ_00053641 -->

    <owl:NamedIndividual rdf:about="http://purl.obolibrary.org/obo/GAZ_00053641">
        <obo:RO_0001025 rdf:resource="http://purl.obolibrary.org/obo/GAZ_00000567"/>
        <obo:IAO_0000115>A broad shield volcano that rises above the NW shore of Lake Abbe (also known as Lake Abhe) in eastern Ethiopia. The 25 km wide volcano was constructed at the southern end of the Kalo Plain. Nested circular craters are located at the summit of the dominantly basaltic volcano, which also displays an older caldera rim. An arcuate chain of rhyolitic lava domes occupies the northern, western, and southern flanks. Youthful basaltic lava flows surround these domes and blanket the flanks of the volcano, and recent flows cover the young sediments of the Kalo and Abhe basins.</obo:IAO_0000115>
        <oboInOwl:hasOBONamespace>GAZ</oboInOwl:hasOBONamespace>
        <oboInOwl:id>GAZ:00053641</oboInOwl:id>
        <rdfs:label>Dama Ali Volcano</rdfs:label>
    </owl:NamedIndividual>
    


    <!-- http://purl.obolibrary.org/obo/GAZ_00053642 -->

    <owl:NamedIndividual rdf:about="http://purl.obolibrary.org/obo/GAZ_00053642">
        <obo:RO_0001025 rdf:resource="http://purl.obolibrary.org/obo/GAZ_00000779"/>
        <obo:IAO_0000115>A rhyolitic stratovolcano along the axis of the Addado graben. The volcano was constructed at the intersection of the central Afar rift zone with the northern end of the NE-SW-trending Ethiopian rift. Rhyolitic lava domes are located on the flanks of the volcano, and a 5 x 17 km basaltic lava field that covers the Ado Bad plain north of the volcano originated from a broad area of fissure vents and spatter cones on the north side of Gabillema volcano. Young lava flows also occur south and east of the volcano, the latter along E-W-trending fissures.</obo:IAO_0000115>
        <oboInOwl:hasOBONamespace>GAZ</oboInOwl:hasOBONamespace>
        <oboInOwl:id>GAZ:00053642</oboInOwl:id>
        <rdfs:label>Gabillema Volcano</rdfs:label>
    </owl:NamedIndividual>
    


    <!-- http://purl.obolibrary.org/obo/GAZ_00053643 -->

    <owl:NamedIndividual rdf:about="http://purl.obolibrary.org/obo/GAZ_00053643">
        <obo:RO_0001025 rdf:resource="http://purl.obolibrary.org/obo/GAZ_00076369"/>
        <obo:IAO_0000115>A complex volcano, lying in the Addado graben of the northern Ethiopian rift, is a complex rhyolitic stratovolcano with an elliptical summit caldera. A trachytic lava flow originating in the caldera covers part of the southern flank. Rhyolitic obsidian domes on the NW flank are surrounded by younger basaltic lava flows. Very recent scoria cones and lava flows are located south of Yangudi along the eastern graben faults.</obo:IAO_0000115>
        <oboInOwl:hasOBONamespace>GAZ</oboInOwl:hasOBONamespace>
        <oboInOwl:id>GAZ:00053643</oboInOwl:id>
        <rdfs:label>Yangudi Volcano</rdfs:label>
    </owl:NamedIndividual>
    


    <!-- http://purl.obolibrary.org/obo/GAZ_00053645 -->

    <owl:NamedIndividual rdf:about="http://purl.obolibrary.org/obo/GAZ_00053645">
        <obo:RO_0001025 rdf:resource="http://purl.obolibrary.org/obo/GAZ_00000779"/>
        <obo:IAO_0000115>A stratovolcano in the southern Afar area immediately east of Ayelu volcano. Adwa is younger than the vegetated Ayelu and is a stratovolcano with a 4 x 5 km caldera that originated following eruption of voluminous ignimbrites. A small 2.5 km wide caldera cuts a trachytic dome extruded in the older caldera. Scoria cones are located on the floor of a circular summit caldera and on its NW and SW flanks. Extensive young basaltic lava flows cover the flanks of Adwa and overlap a sedimentary plain to the SE. Many fumaroles occur within the caldera of Adwa.</obo:IAO_0000115>
        <oboInOwl:hasOBONamespace>GAZ</oboInOwl:hasOBONamespace>
        <oboInOwl:id>GAZ:00053645</oboInOwl:id>
        <rdfs:label>Adwa Volcano</rdfs:label>
    </owl:NamedIndividual>
    


    <!-- http://purl.obolibrary.org/obo/GAZ_00053646 -->

    <owl:NamedIndividual rdf:about="http://purl.obolibrary.org/obo/GAZ_00053646">
        <obo:RO_0001025 rdf:resource="http://purl.obolibrary.org/obo/GAZ_00000567"/>
        <obo:IAO_0000115>A basaltic fissure vent that fed lava flows at the south end of the Awash plain, about 50 km NNE of Dofen volcano.</obo:IAO_0000115>
        <oboInOwl:hasOBONamespace>GAZ</oboInOwl:hasOBONamespace>
        <oboInOwl:id>GAZ:00053646</oboInOwl:id>
        <rdfs:label>Hertali Volcano</rdfs:label>
    </owl:NamedIndividual>
    


    <!-- http://purl.obolibrary.org/obo/GAZ_00053647 -->

    <owl:NamedIndividual rdf:about="http://purl.obolibrary.org/obo/GAZ_00053647">
        <obo:RO_0001025 rdf:resource="http://purl.obolibrary.org/obo/GAZ_00000567"/>
        <obo:IAO_0000115>A volcanic field (maars) that consists of a dozen closely spaced maars and cinder cones with associated lava fields in the Awash plain NE of Dofen volcano.</obo:IAO_0000115>
        <oboInOwl:hasOBONamespace>GAZ</oboInOwl:hasOBONamespace>
        <oboInOwl:id>GAZ:00053647</oboInOwl:id>
        <rdfs:label>Liado Hayk Volcanic Field</rdfs:label>
    </owl:NamedIndividual>
    


    <!-- http://purl.obolibrary.org/obo/GAZ_00053648 -->

    <owl:NamedIndividual rdf:about="http://purl.obolibrary.org/obo/GAZ_00053648">
        <obo:RO_0001025 rdf:resource="http://purl.obolibrary.org/obo/GAZ_00000779"/>
        <obo:IAO_0000115>One of the 29 woredas in the Afar Region of Ethiopia. Because Argobba is not part of any Zone in the Afar Region, it is considered a Special woreda.</obo:IAO_0000115>
        <oboInOwl:hasOBONamespace>GAZ</oboInOwl:hasOBONamespace>
        <oboInOwl:id>GAZ:00053648</oboInOwl:id>
        <rdfs:label>Argobba Special Woreda</rdfs:label>
    </owl:NamedIndividual>
    


    <!-- http://purl.obolibrary.org/obo/GAZ_00053649 -->

    <owl:NamedIndividual rdf:about="http://purl.obolibrary.org/obo/GAZ_00053649">
        <obo:RO_0001025 rdf:resource="http://purl.obolibrary.org/obo/GAZ_00000779"/>
        <obo:IAO_0000115>A 1151 m high stratovolcano that rises 450 m above the Awash plain in the northern Main Ethiopian Rift. Numerous cinder cones, constructed along a 10 km-long, N-S-trending line, dot the flanks of the dominantly rhyolitic volcano. The northern cones are younger, have well-preserved morphologies, and display strong fumarolic activity. A major fumarole in a wide south-flank crater has precipitated large amounts of sulfur.</obo:IAO_0000115>
        <oboInOwl:hasOBONamespace>GAZ</oboInOwl:hasOBONamespace>
        <oboInOwl:id>GAZ:00053649</oboInOwl:id>
        <rdfs:label>Dofen Volcano</rdfs:label>
    </owl:NamedIndividual>
    


    <!-- http://purl.obolibrary.org/obo/GAZ_00053650 -->

    <owl:NamedIndividual rdf:about="http://purl.obolibrary.org/obo/GAZ_00053650">
        <obo:RO_0001025 rdf:resource="http://purl.obolibrary.org/obo/GAZ_00123874"/>
        <obo:IAO_0000115>A large stratovolcano at the northern end of the Main Ethiopian Rift. It consists primarily of rhyolitic obsidian lava flows with minor tuffs. Welded pantelleritic ash flows accompanied formation of a 2.5 x 4.5 km summit caldera, which has steep-sided walls up to 500 m high. The WNW-ESE-trending elliptical caldera has an orientation perpendicular to the Ethiopian Rift, and post-caldera vents occur along the same orientation. Trachytic and obsidian lava flows occur on the caldera floor, and fresh-looking lava flows descend the flanks from satellitic vents.</obo:IAO_0000115>
        <oboInOwl:hasOBONamespace>GAZ</oboInOwl:hasOBONamespace>
        <oboInOwl:id>GAZ:00053650</oboInOwl:id>
        <rdfs:label>Mount Fentale</rdfs:label>
    </owl:NamedIndividual>
    


    <!-- http://purl.obolibrary.org/obo/GAZ_00053651 -->

    <owl:NamedIndividual rdf:about="http://purl.obolibrary.org/obo/GAZ_00053651">
        <obo:RO_0001025 rdf:resource="http://purl.obolibrary.org/obo/GAZ_00000567"/>
        <obo:IAO_0000115>An area of Holocene basaltic lava flows is located along the Main Ethiopian Rift at Beru, between Fentale and Kone (Gariboldi) volcanoes.</obo:IAO_0000115>
        <oboInOwl:hasOBONamespace>GAZ</oboInOwl:hasOBONamespace>
        <oboInOwl:id>GAZ:00053651</oboInOwl:id>
        <rdfs:label>Beru Volcanic Field</rdfs:label>
    </owl:NamedIndividual>
    


    <!-- http://purl.obolibrary.org/obo/GAZ_00053652 -->

    <owl:NamedIndividual rdf:about="http://purl.obolibrary.org/obo/GAZ_00053652">
        <obo:RO_0001025 rdf:resource="http://purl.obolibrary.org/obo/GAZ_00000784"/>
        <obo:IAO_0000115>Calderas composed of a series of silicic calderas and young basaltic cinder cones and lava flows about 30 km SW of Fentale volcano. As many as eight silicic calderas are accompanied by ignimbrite outflow sheets. Gariboldi, the youngest caldera, is an elliptical 5 x 7.5 km wide caldera trending E-W and oriented perpendicular to the Main Ethiopian Rift. The rim of the caldera rises about 100 m above the caldera floor; the eastern rim overlaps with a smaller elliptical caldera. Roughly N-S-trending regional fissures cut across the caldera and its flanks.</obo:IAO_0000115>
        <oboInOwl:hasOBONamespace>GAZ</oboInOwl:hasOBONamespace>
        <oboInOwl:id>GAZ:00053652</oboInOwl:id>
        <rdfs:label>Kone Volcanic Complex</rdfs:label>
    </owl:NamedIndividual>
    


    <!-- http://purl.obolibrary.org/obo/GAZ_00053653 -->

    <owl:NamedIndividual rdf:about="http://purl.obolibrary.org/obo/GAZ_00053653">
        <obo:RO_0001025 rdf:resource="http://purl.obolibrary.org/obo/GAZ_00000567"/>
        <obo:IAO_0000115>A composite dominantly rhyolitic-to-trachytic stratovolcanoes rising 1000 m and 800 m, respectively, above the floor of the Ethiopian Rift valley. Initial basaltic-to-trachytic activity at Boset was followed by rhyolitic effusive and explosive eruptions that resulted in caldera formation. A remnant of the caldera rim is found on the NW flank of Boset. Elsewhere post-caldera activity has produced very recent pantelleritic obsidian fissure-fed lava domes and flows that have buried the caldera wall, and flank eruptions from fissures parallel to the rift have produced voluminous pantelleritic lava flows. Bericha has produced similar very recent obsidian flows and associated pumice flows. Fissures connecting Boset and Bericha have erupted youthful, prehistorical basaltic lava flows.</obo:IAO_0000115>
        <oboInOwl:hasOBONamespace>GAZ</oboInOwl:hasOBONamespace>
        <oboInOwl:id>GAZ:00053653</oboInOwl:id>
        <rdfs:label>Boset-Bericha Volcanic Complex</rdfs:label>
    </owl:NamedIndividual>
    


    <!-- http://purl.obolibrary.org/obo/GAZ_00053654 -->

    <owl:NamedIndividual rdf:about="http://purl.obolibrary.org/obo/GAZ_00053654">
        <obo:RO_0001025 rdf:resource="http://purl.obolibrary.org/obo/GAZ_00053653"/>
        <obo:IAO_0000115>A stratovolcano.</obo:IAO_0000115>
        <oboInOwl:hasOBONamespace>GAZ</oboInOwl:hasOBONamespace>
        <oboInOwl:id>GAZ:00053654</oboInOwl:id>
        <rdfs:label>Boset Volcano</rdfs:label>
    </owl:NamedIndividual>
    


    <!-- http://purl.obolibrary.org/obo/GAZ_00053655 -->

    <owl:NamedIndividual rdf:about="http://purl.obolibrary.org/obo/GAZ_00053655">
        <obo:RO_0001025 rdf:resource="http://purl.obolibrary.org/obo/GAZ_00053653"/>
        <obo:IAO_0000115>A stratovolcano.</obo:IAO_0000115>
        <oboInOwl:hasOBONamespace>GAZ</oboInOwl:hasOBONamespace>
        <oboInOwl:id>GAZ:00053655</oboInOwl:id>
        <rdfs:label>Bericha Volcano</rdfs:label>
    </owl:NamedIndividual>
    


    <!-- http://purl.obolibrary.org/obo/GAZ_00053656 -->

    <owl:NamedIndividual rdf:about="http://purl.obolibrary.org/obo/GAZ_00053656">
        <obo:RO_0001025 rdf:resource="http://purl.obolibrary.org/obo/GAZ_00000784"/>
        <obo:IAO_0000115>An area of fissure-fed Holocene lava flows, cinder cones, tuff rings, and maars. Several of the maars are filled by lakes. Most of the craters and cones are aligned NE-SW, parallel to the direction of the Ethiopian Rift Valley. The 750 x 1000 m wide Haro Maja tuff ring and its neighbor, lake-filled Kilole, are offset to the east. The cones and maars of the Bishoftu volcanic field were erupted through rhyolitic welded tuffs.</obo:IAO_0000115>
        <oboInOwl:hasOBONamespace>GAZ</oboInOwl:hasOBONamespace>
        <oboInOwl:id>GAZ:00053656</oboInOwl:id>
        <rdfs:label>Bishoftu Volcanic Field</rdfs:label>
    </owl:NamedIndividual>
    


    <!-- http://purl.obolibrary.org/obo/GAZ_00053657 -->

    <owl:NamedIndividual rdf:about="http://purl.obolibrary.org/obo/GAZ_00053657">
        <obo:RO_0001025 rdf:resource="http://purl.obolibrary.org/obo/GAZ_00000567"/>
        <obo:IAO_0000115>A volcanic field that is an extensive 15 x 25 km wide group of Pleistocene and Holocene pyroclastic cones and lava flows that covers the floor of the eastern side of the Ethiopian Rift Valley, north of the town of Malkassa, between Boset-Bericha and Gedamsa volcanoes. The basaltic lava flows extend beyond the western flanks of Boset and Bericha volcanoes as far north as the village of Welenchiti.</obo:IAO_0000115>
        <oboInOwl:hasOBONamespace>GAZ</oboInOwl:hasOBONamespace>
        <oboInOwl:id>GAZ:00053657</oboInOwl:id>
        <rdfs:label>Sodore Volcanic Field</rdfs:label>
    </owl:NamedIndividual>
    


    <!-- http://purl.obolibrary.org/obo/GAZ_00053658 -->

    <owl:NamedIndividual rdf:about="http://purl.obolibrary.org/obo/GAZ_00053658">
        <obo:RO_0001025 rdf:resource="http://purl.obolibrary.org/obo/GAZ_00000567"/>
        <obo:IAO_0000115>A caldera located along the Main Ethiopian Rift east of Lake Koka and SW of the Wonji Sugar Estate Farm. The 7 x 9 km wide caldera (also spelled Gadamsa or Gedemsa) is cut by many NNE-SSW-trending regional faults of the Ethiopian Rift, particularly on the east side of the caldera. The caldera is steep-sided, with 100-200 m high walls whose upper part consists primarily of rhyolitic lava flows, and formed as a result of the eruption of a series of trachytic ignimbrites. Late-Pleistocene to Holocene volcanics form a chain of rhyolitic lava flows and pumice deposits, known as Ittisa, that rises about 200-250 m above the floor of the caldera. A large 1 km wide crater is located at the eastern part of the chain. A Holocene lava dome or flow is found on the SW flank of the volcano. Regional faults have truncated the volcano, and small basaltic spatter cones have formed inside the caldera rim. Weak fumarolic activity was reported at two locations at Gedamsa.</obo:IAO_0000115>
        <oboInOwl:hasOBONamespace>GAZ</oboInOwl:hasOBONamespace>
        <oboInOwl:id>GAZ:00053658</oboInOwl:id>
        <rdfs:label>Gedamsa Caldera</rdfs:label>
    </owl:NamedIndividual>
    


    <!-- http://purl.obolibrary.org/obo/GAZ_00053659 -->

    <owl:NamedIndividual rdf:about="http://purl.obolibrary.org/obo/GAZ_00053659">
        <obo:RO_0001025 rdf:resource="http://purl.obolibrary.org/obo/GAZ_00000567"/>
        <obo:IAO_0000115>Pumice cones that rise 350-500 m above the floor of the rift. Bora has a 1.5 km wide summit crater, and the more conical Bericcio is capped by a small summit crater and has a 1 km wide crater on its south flank. Small silicic pyroclastic cones are found on the east flanks of both Bora and Bericcio. All volcanic products in this area are considered to be Holocene in age. Vigorous fumarolic activity continues at Bora-Bericcio.</obo:IAO_0000115>
        <oboInOwl:hasOBONamespace>GAZ</oboInOwl:hasOBONamespace>
        <oboInOwl:id>GAZ:00053659</oboInOwl:id>
        <rdfs:label>Bora-Bericcio Pumice Cones</rdfs:label>
    </owl:NamedIndividual>
    


    <!-- http://purl.obolibrary.org/obo/GAZ_00053660 -->

    <owl:NamedIndividual rdf:about="http://purl.obolibrary.org/obo/GAZ_00053660">
        <obo:RO_0001025 rdf:resource="http://purl.obolibrary.org/obo/GAZ_00000567"/>
        <obo:IAO_0000115>A youthful trachytic-to-rhyolitic pumice cone with a 700-m-wide summit crater, located in the middle of one of the most active parts of the Ethiopian Rift Valley. A large silicic lava flow at Giano was erupted about two centuries ago from a regional fissure. Flank fissures have produced silicic lava flows as recently as about 1900 AD. The same fissures have also erupted prehistorical basaltic lava flows.</obo:IAO_0000115>
        <oboInOwl:hasOBONamespace>GAZ</oboInOwl:hasOBONamespace>
        <oboInOwl:id>GAZ:00053660</oboInOwl:id>
        <rdfs:label>Tullu Moje Pumice Cone</rdfs:label>
    </owl:NamedIndividual>
    


    <!-- http://purl.obolibrary.org/obo/GAZ_00053661 -->

    <owl:NamedIndividual rdf:about="http://purl.obolibrary.org/obo/GAZ_00053661">
        <obo:RO_0001025 rdf:resource="http://purl.obolibrary.org/obo/GAZ_00000567"/>
        <obo:IAO_0000115>A large area of Recent-to-prehistorical basaltic cinder cones and lava flows that lies immediately east and south of Lake Zway (also spelled Zwai, Zeway, and Ziway) and forms islands along the east shore of the lake. About 80 vents were formed along the East Zway segment of the Wonji Fault Belt. The youngest lava flows at East Zway are unaffected by the latest tectonic faulting along the Ethiopian Rift.</obo:IAO_0000115>
        <oboInOwl:hasOBONamespace>GAZ</oboInOwl:hasOBONamespace>
        <oboInOwl:id>GAZ:00053661</oboInOwl:id>
        <rdfs:label>East Zway Fissure Vents</rdfs:label>
    </owl:NamedIndividual>
    


    <!-- http://purl.obolibrary.org/obo/GAZ_00053662 -->

    <owl:NamedIndividual rdf:about="http://purl.obolibrary.org/obo/GAZ_00053662">
        <obo:RO_0001025 rdf:resource="http://purl.obolibrary.org/obo/GAZ_00000567"/>
        <obo:IAO_0000115>A volcanic field that onsists of a large group of basaltic cinder cones, maars, and lava flows in an 80 km-long, NE-SW-trending area near the west margin of the Ethiopian Rift. At least 13 maars, many filled by lakes, are located near the town of Debre Zeit, SE of the capital city of Addis Ababa. The maars were erupted through Pleistocene rhyolitic lava flows and tuffs. Eruptions of the younger basaltic cinder cones were contemporaneous with those that produced the maars.</obo:IAO_0000115>
        <oboInOwl:hasOBONamespace>GAZ</oboInOwl:hasOBONamespace>
        <oboInOwl:id>GAZ:00053662</oboInOwl:id>
        <rdfs:label>Butajiri-Silti Volcanic Field</rdfs:label>
    </owl:NamedIndividual>
    


    <!-- http://purl.obolibrary.org/obo/GAZ_00053663 -->

    <owl:NamedIndividual rdf:about="http://purl.obolibrary.org/obo/GAZ_00053663">
        <obo:RO_0001025 rdf:resource="http://purl.obolibrary.org/obo/GAZ_00000007"/>
        <obo:RO_0001025 rdf:resource="http://purl.obolibrary.org/obo/GAZ_00123873"/>
        <obo:IAO_0000115>A freshwater lake in the Oromia Region of Ethiopia, about 100 km south of the capital, Addis Ababa, on the border between the Misraq Shewa and Arsi Zones. It is located in the Great Rift Valley at an elevation of 1,585 meters to the east of Lake Abijatta.</obo:IAO_0000115>
        <oboInOwl:hasOBONamespace>GAZ</oboInOwl:hasOBONamespace>
        <oboInOwl:id>GAZ:00053663</oboInOwl:id>
        <rdfs:label>Lake Langano</rdfs:label>
    </owl:NamedIndividual>
    


    <!-- http://purl.obolibrary.org/obo/GAZ_00053664 -->

    <owl:NamedIndividual rdf:about="http://purl.obolibrary.org/obo/GAZ_00053664">
        <obo:RO_0001025 rdf:resource="http://purl.obolibrary.org/obo/GAZ_00000784"/>
        <obo:IAO_0000115>A stratovolcano with multiple vents aligned along NNE-SSW and E-W fissures along a narrow graben between the two lakes. This silicic volcanic center lies along the regional Wonji Fault Belt and has produced abundant pumice-flow and pumice-fall deposits, along with lesser rhyolitic lava flows. Obsidian lava flows erupted from craters along the fissures have descended the flanks in all directions. Cinder cones, lava domes, phreatic explosion craters, and thermal springs are structurally controlled.</obo:IAO_0000115>
        <oboInOwl:hasOBONamespace>GAZ</oboInOwl:hasOBONamespace>
        <oboInOwl:id>GAZ:00053664</oboInOwl:id>
        <rdfs:label>Alutu Volcano</rdfs:label>
    </owl:NamedIndividual>
    


    <!-- http://purl.obolibrary.org/obo/GAZ_00053665 -->

    <owl:NamedIndividual rdf:about="http://purl.obolibrary.org/obo/GAZ_00053665">
        <obo:RO_0001025 rdf:resource="http://purl.obolibrary.org/obo/GAZ_00053666"/>
        <obo:IAO_0000115>A caldera that forms the eastern portion of the 15 x 25 km dumbbell-shaped Lake O&apos;a (also known as Lake Shalla). Formation of the caldera about 240,000 years ago was accompanied by the eruption of two ignimbrite deposits, the first of which was strongly welded. The only post-caldera activity consists of two pyroclastic cones north of the caldera, one silicic and the other basaltic, and a group of tuff rings, spatter cones, and lava flows of Holocene (perhaps as young as prehistorical) age near the SW shore of the lake. These were erupted along the Corbetti-Shalla segment of the Wonji Fault Belt, which extends north from Corbetti caldera. Fumarolic activity continues on all sides of the lake.</obo:IAO_0000115>
        <oboInOwl:hasOBONamespace>GAZ</oboInOwl:hasOBONamespace>
        <oboInOwl:id>GAZ:00053665</oboInOwl:id>
        <rdfs:label>O&apos;a Caldera</rdfs:label>
    </owl:NamedIndividual>
    


    <!-- http://purl.obolibrary.org/obo/GAZ_00053666 -->

    <owl:NamedIndividual rdf:about="http://purl.obolibrary.org/obo/GAZ_00053666">
        <obo:RO_0001025 rdf:resource="http://purl.obolibrary.org/obo/GAZ_00000784"/>
        <obo:IAO_0000115>A national park located in the Oromia Region 200 km south of Addis Ababa to the east of the Ziway to Shashamane highway, it contains 887 km2 including the Rift Valley lakes of Abijatta and Shalla. The two lakes are separated by three km of hilly land.</obo:IAO_0000115>
        <oboInOwl:hasOBONamespace>GAZ</oboInOwl:hasOBONamespace>
        <oboInOwl:id>GAZ:00053666</oboInOwl:id>
        <rdfs:label>Abijatta-Shalla National Park</rdfs:label>
    </owl:NamedIndividual>
    


    <!-- http://purl.obolibrary.org/obo/GAZ_00053667 -->

    <owl:NamedIndividual rdf:about="http://purl.obolibrary.org/obo/GAZ_00053667">
        <obo:RO_0001025 rdf:resource="http://purl.obolibrary.org/obo/GAZ_00000007"/>
        <obo:RO_0001025 rdf:resource="http://purl.obolibrary.org/obo/GAZ_00053666"/>
        <obo:IAO_0000115>A lake that is surrounded by hot springs filled with boiling water, and the earth surrounding the lake is filled with cracks due to erosion and earthquakes. Due to steam rising from the boiling water in the springs, the atmosphere around the lake is relatively foggy.</obo:IAO_0000115>
        <oboInOwl:hasOBONamespace>GAZ</oboInOwl:hasOBONamespace>
        <oboInOwl:id>GAZ:00053667</oboInOwl:id>
        <rdfs:label>Lake Shala</rdfs:label>
    </owl:NamedIndividual>
    


    <!-- http://purl.obolibrary.org/obo/GAZ_00053668 -->

    <owl:NamedIndividual rdf:about="http://purl.obolibrary.org/obo/GAZ_00053668">
        <obo:RO_0001025 rdf:resource="http://purl.obolibrary.org/obo/GAZ_00053667"/>
        <obo:IAO_0000115>An island in Lake Shala.</obo:IAO_0000115>
        <oboInOwl:hasOBONamespace>GAZ</oboInOwl:hasOBONamespace>
        <oboInOwl:id>GAZ:00053668</oboInOwl:id>
        <rdfs:label>Pelican Island</rdfs:label>
    </owl:NamedIndividual>
    


    <!-- http://purl.obolibrary.org/obo/GAZ_00053669 -->

    <owl:NamedIndividual rdf:about="http://purl.obolibrary.org/obo/GAZ_00053669">
        <obo:RO_0001025 rdf:resource="http://purl.obolibrary.org/obo/GAZ_00000567"/>
        <obo:IAO_0000115>A volcanic field that contains a group of lake-filled maars and tuff rings of Pleistocene and probable Holocene age. Active hot springs and fumaroles are located in this area.</obo:IAO_0000115>
        <oboInOwl:hasOBONamespace>GAZ</oboInOwl:hasOBONamespace>
        <oboInOwl:id>GAZ:00053669</oboInOwl:id>
        <rdfs:label>Bilate River Volcanic Field</rdfs:label>
    </owl:NamedIndividual>
    


    <!-- http://purl.obolibrary.org/obo/GAZ_00053670 -->

    <owl:NamedIndividual rdf:about="http://purl.obolibrary.org/obo/GAZ_00053670">
        <obo:RO_0001025 rdf:resource="http://purl.obolibrary.org/obo/GAZ_00123648"/>
        <obo:IAO_0000115>A basaltic shield volcano, morphologically unmodified in a region of high rainfall. It is capped by prominent cinder cones and small craters. Three satellitic centers are located along an E-W line north of the main shield, whose 2728 m high summit forms Ethiopia&apos;s highest Holocene volcano. Lava flows have traveled down pre-existing valleys. Tepi lies at the northern end of the Turkana rift, about 300 km west of the center of the main Ethiopian rift and was constructed along a zone of ENE-trending faults that extends in line with the Gulf of Aden. Tepi has associated active hot springs.</obo:IAO_0000115>
        <oboInOwl:hasOBONamespace>GAZ</oboInOwl:hasOBONamespace>
        <oboInOwl:id>GAZ:00053670</oboInOwl:id>
        <rdfs:label>Tepi Volcano</rdfs:label>
    </owl:NamedIndividual>
    


    <!-- http://purl.obolibrary.org/obo/GAZ_00053671 -->

    <owl:NamedIndividual rdf:about="http://purl.obolibrary.org/obo/GAZ_00053671">
        <obo:RO_0001025 rdf:resource="http://purl.obolibrary.org/obo/GAZ_00053672"/>
        <obo:IAO_0000115>A large caldera of Pleistocene age. Fissures cutting the SE margin of the caldera produced numerous pyroclastic cones of Pleistocene-to-Holocene age.</obo:IAO_0000115>
        <oboInOwl:hasOBONamespace>GAZ</oboInOwl:hasOBONamespace>
        <oboInOwl:id>GAZ:00053671</oboInOwl:id>
        <rdfs:label>Hobicha Caldera</rdfs:label>
    </owl:NamedIndividual>
    


    <!-- http://purl.obolibrary.org/obo/GAZ_00053672 -->

    <owl:NamedIndividual rdf:about="http://purl.obolibrary.org/obo/GAZ_00053672">
        <obo:RO_0001025 rdf:resource="http://purl.obolibrary.org/obo/GAZ_00000567"/>
        <obo:IAO_0000115>A volcanic field.</obo:IAO_0000115>
        <oboInOwl:hasOBONamespace>GAZ</oboInOwl:hasOBONamespace>
        <oboInOwl:id>GAZ:00053672</oboInOwl:id>
        <rdfs:label>Northern Lake Abaya Volcanic Field</rdfs:label>
    </owl:NamedIndividual>
    


    <!-- http://purl.obolibrary.org/obo/GAZ_00053673 -->

    <owl:NamedIndividual rdf:about="http://purl.obolibrary.org/obo/GAZ_00053673">
        <obo:RO_0001025 rdf:resource="http://purl.obolibrary.org/obo/GAZ_00000567"/>
        <obo:IAO_0000115>A rhyolitic stratovolcano located on the Wonji fault belt NE of Lake Abaya. All rift zone volcanoes are thought to be Pleistocene-to-Holocene in age, with the possible exception of Chiracha, which may be pre-Holocene.</obo:IAO_0000115>
        <oboInOwl:hasOBONamespace>GAZ</oboInOwl:hasOBONamespace>
        <oboInOwl:id>GAZ:00053673</oboInOwl:id>
        <rdfs:label>Chiracha Volcano</rdfs:label>
    </owl:NamedIndividual>
    


    <!-- http://purl.obolibrary.org/obo/GAZ_00053674 -->

    <owl:NamedIndividual rdf:about="http://purl.obolibrary.org/obo/GAZ_00053674">
        <obo:RO_0001025 rdf:resource="http://purl.obolibrary.org/obo/GAZ_00000786"/>
        <obo:IAO_0000115>A group of cinder cones at Tosa Sucha on the north shore of Lake Chamo in the southern Ethiopian Rift has produced unvegetated olivine basaltic lava flows and may have been active as recently as historical time. The cones and flows on the eastern end of the Chamo Basin were erupted along NNE-trending fissures between Lake Chamo and Lake Abaya to the north. Some cones form islands in Lake Chamo.</obo:IAO_0000115>
        <oboInOwl:hasOBONamespace>GAZ</oboInOwl:hasOBONamespace>
        <oboInOwl:id>GAZ:00053674</oboInOwl:id>
        <rdfs:label>Tosa Sucha Cinder Cones</rdfs:label>
    </owl:NamedIndividual>
    


    <!-- http://purl.obolibrary.org/obo/GAZ_00053675 -->

    <owl:NamedIndividual rdf:about="http://purl.obolibrary.org/obo/GAZ_00053675">
        <obo:RO_0001025 rdf:resource="http://purl.obolibrary.org/obo/GAZ_00000007"/>
        <obo:RO_0001025 rdf:resource="http://purl.obolibrary.org/obo/GAZ_00053676"/>
        <obo:RO_0001025 rdf:resource="http://purl.obolibrary.org/obo/GAZ_00123681"/>
        <obo:IAO_0000115>A lake in the Southern Nations, Nationalities, and Peoples Region of southern Ethiopia. It is located in the Great Rift Valley at an elevation of 1,235 meters. It is just to the south of Lake Abaya and the city of Arba Minch, and east of the Guge Mountains. Lake Chamo does not always have an outflow, but in some years, it overflows into the Sagan River. In some years, it is fed by overflow from Lake Abaya.</obo:IAO_0000115>
        <oboInOwl:hasOBONamespace>GAZ</oboInOwl:hasOBONamespace>
        <oboInOwl:id>GAZ:00053675</oboInOwl:id>
        <rdfs:label>Lake Chamo</rdfs:label>
    </owl:NamedIndividual>
    


    <!-- http://purl.obolibrary.org/obo/GAZ_00053676 -->

    <owl:NamedIndividual rdf:about="http://purl.obolibrary.org/obo/GAZ_00053676">
        <obo:RO_0001025 rdf:resource="http://purl.obolibrary.org/obo/GAZ_00000786"/>
        <obo:IAO_0000115>A national park located in the Southern Nations, Nationalities, and Peoples Region immediately to the east of Arba Minch, its 514 km2 of territory include the &quot;Bridge of God&quot; (an isthmus between Lakes Abaya and Chamo), and the Nechisar plains east of the lakes.</obo:IAO_0000115>
        <oboInOwl:hasOBONamespace>GAZ</oboInOwl:hasOBONamespace>
        <oboInOwl:id>GAZ:00053676</oboInOwl:id>
        <rdfs:label>Nechisar National Park</rdfs:label>
    </owl:NamedIndividual>
    


    <!-- http://purl.obolibrary.org/obo/GAZ_00053677 -->

    <owl:NamedIndividual rdf:about="http://purl.obolibrary.org/obo/GAZ_00053677">
        <obo:RO_0001025 rdf:resource="http://purl.obolibrary.org/obo/GAZ_00000567"/>
        <obo:IAO_0000115>An isolated group of tuff cones and lava flows in southern Ethiopia that were erupted along the Turkana Rift, which extends north from Kenya. About 20 tuff cones occupy the Korath Range, many of which issued lava flows from their flanks that traveled up to about 5 km. The apparent youngest flow issued from the central crater and flowed through a breach in its rim.</obo:IAO_0000115>
        <oboInOwl:hasOBONamespace>GAZ</oboInOwl:hasOBONamespace>
        <oboInOwl:id>GAZ:00053677</oboInOwl:id>
        <rdfs:label>Korath Range</rdfs:label>
    </owl:NamedIndividual>
    


    <!-- http://purl.obolibrary.org/obo/GAZ_00053679 -->

    <owl:NamedIndividual rdf:about="http://purl.obolibrary.org/obo/GAZ_00053679">
        <obo:RO_0001025 rdf:resource="http://purl.obolibrary.org/obo/GAZ_00000779"/>
        <obo:RO_0001025 rdf:resource="http://purl.obolibrary.org/obo/GAZ_00051205"/>
        <obo:RO_0001025 rdf:resource="http://purl.obolibrary.org/obo/GAZ_00123426"/>
        <obo:IAO_0000115>A vegetated rhyolitic stratovolcano, located south of the Asbahri plain in the southern Afar region. On its eastern side, 2145 m high Ayelu is cut by regional faults and is overlain by ignimbrites erupted from Adwa volcano immediately to the east. Ayelu was constructed by a series of thick rhyolitic lava flows, creating a higher and steeper-sided volcano than its neighbor Adwa. Hot springs are located on the western flank of Ayelu.</obo:IAO_0000115>
        <oboInOwl:hasOBONamespace>GAZ</oboInOwl:hasOBONamespace>
        <oboInOwl:id>GAZ:00053679</oboInOwl:id>
        <rdfs:label>Mount Ayalu</rdfs:label>
    </owl:NamedIndividual>
    


    <!-- http://purl.obolibrary.org/obo/GAZ_00053680 -->

    <owl:NamedIndividual rdf:about="http://purl.obolibrary.org/obo/GAZ_00053680">
        <obo:RO_0001025 rdf:resource="http://purl.obolibrary.org/obo/GAZ_00053681"/>
        <obo:IAO_0000115>An extinct volcano in the Oromia region of Ethiopia. Situated in Ada&apos;a Chukala woreda of the Misraq (East) Shewa Zone, it rises from the plain 30 km south of Debre Zeyit.</obo:IAO_0000115>
        <oboInOwl:hasOBONamespace>GAZ</oboInOwl:hasOBONamespace>
        <oboInOwl:id>GAZ:00053680</oboInOwl:id>
        <rdfs:label>Mount Zuqualla</rdfs:label>
    </owl:NamedIndividual>
    


    <!-- http://purl.obolibrary.org/obo/GAZ_00053681 -->

    <owl:NamedIndividual rdf:about="http://purl.obolibrary.org/obo/GAZ_00053681">
        <obo:RO_0001025 rdf:resource="http://purl.obolibrary.org/obo/GAZ_00031119"/>
        <obo:IAO_0000115>One of the 180 woredas in the Oromia Region of Ethiopia. Part of the Misraq Shewa Zone located in the Great Rift Valley, Ada&apos;a Chukala is bordered on the south by Dugda Bora, on the west by the Mirab Shewa Zone, on the northwest by Akaki, on the northeast by Gimbichu, and on the east by Lome. The capital is Debre Zeit; other towns in Ada&apos;a Chukala include Adulala.</obo:IAO_0000115>
        <oboInOwl:hasOBONamespace>GAZ</oboInOwl:hasOBONamespace>
        <oboInOwl:id>GAZ:00053681</oboInOwl:id>
        <rdfs:label>Ada&apos;a Chukala Woreda</rdfs:label>
    </owl:NamedIndividual>
    


    <!-- http://purl.obolibrary.org/obo/GAZ_00057510 -->

    <owl:NamedIndividual rdf:about="http://purl.obolibrary.org/obo/GAZ_00057510">
        <obo:RO_0001025 rdf:resource="http://purl.obolibrary.org/obo/GAZ_00051205"/>
        <obo:RO_0001025 rdf:resource="http://purl.obolibrary.org/obo/GAZ_00123420"/>
        <obo:IAO_0000115>An endorheic saline lake lying on the Ethiopia-Djibouti border, and is one of a chain of six connected lakes which also includes (from north to south) lakes Gargori, Laitali, Gummare, Bario and Afambo. Lake Abbe is the ultimate destination of the waters of the Awash River. Lake Abbe is at the central point of the Afar Depression, where three pieces of the earth&apos;s crust meet. On the northwest shore rises Dama Ali, a volcanic mountain.</obo:IAO_0000115>
        <oboInOwl:hasOBONamespace>GAZ</oboInOwl:hasOBONamespace>
        <oboInOwl:id>GAZ:00057510</oboInOwl:id>
        <rdfs:label>Lake Abbe</rdfs:label>
    </owl:NamedIndividual>
    


    <!-- http://purl.obolibrary.org/obo/GAZ_00057758 -->

    <owl:NamedIndividual rdf:about="http://purl.obolibrary.org/obo/GAZ_00057758">
        <obo:RO_0001025 rdf:resource="http://purl.obolibrary.org/obo/GAZ_00000567"/>
        <obo:IAO_0000115>A desert located in north eastern Ethiopia and in southern Eritrea, where it forms the Southern Red Sea district.</obo:IAO_0000115>
        <oboInOwl:hasOBONamespace>GAZ</oboInOwl:hasOBONamespace>
        <oboInOwl:id>GAZ:00057758</oboInOwl:id>
        <rdfs:label>Danakil Desert</rdfs:label>
    </owl:NamedIndividual>
    


    <!-- http://purl.obolibrary.org/obo/GAZ_00058384 -->

    <owl:NamedIndividual rdf:about="http://purl.obolibrary.org/obo/GAZ_00058384">
        <obo:RO_0001025 rdf:resource="http://purl.obolibrary.org/obo/GAZ_00008742"/>
        <obo:IAO_0000115>A lake that was drained in the 1950s, but is now being regenerated.</obo:IAO_0000115>
        <oboInOwl:hasOBONamespace>GAZ</oboInOwl:hasOBONamespace>
        <oboInOwl:id>GAZ:00058384</oboInOwl:id>
        <rdfs:label>Lake Hulah</rdfs:label>
    </owl:NamedIndividual>
    


    <!-- http://purl.obolibrary.org/obo/GAZ_00058395 -->

    <owl:NamedIndividual rdf:about="http://purl.obolibrary.org/obo/GAZ_00058395">
        <obo:RO_0001025 rdf:resource="http://purl.obolibrary.org/obo/GAZ_00058396"/>
        <obo:IAO_0000115>An artificial lake located in the southern region of the Beqaa Valley. Made by damming the Litani River.</obo:IAO_0000115>
        <oboInOwl:hasOBONamespace>GAZ</oboInOwl:hasOBONamespace>
        <oboInOwl:id>GAZ:00058395</oboInOwl:id>
        <rdfs:label>Lake Qaraoun</rdfs:label>
    </owl:NamedIndividual>
    


    <!-- http://purl.obolibrary.org/obo/GAZ_00058396 -->

    <owl:NamedIndividual rdf:about="http://purl.obolibrary.org/obo/GAZ_00058396">
        <obo:RO_0001025 rdf:resource="http://purl.obolibrary.org/obo/GAZ_00044906"/>
        <obo:IAO_0000115>A river that rises west of Baalbek in the fertile Beqaa Valley and empties in the Mediterranean Sea north of Tyre.</obo:IAO_0000115>
        <oboInOwl:hasOBONamespace>GAZ</oboInOwl:hasOBONamespace>
        <oboInOwl:id>GAZ:00058396</oboInOwl:id>
        <rdfs:label>Litani River</rdfs:label>
    </owl:NamedIndividual>
    


    <!-- http://purl.obolibrary.org/obo/GAZ_00058780 -->

    <owl:NamedIndividual rdf:about="http://purl.obolibrary.org/obo/GAZ_00058780">
        <obo:RO_0001025 rdf:resource="http://purl.obolibrary.org/obo/GAZ_00058782"/>
        <obo:IAO_0000115>A lake lagoon in Zambia. It is the largest of several lagoons in the Luapula River swamps south of Lake Mweru, in the Luapula Province of Zambia.</obo:IAO_0000115>
        <oboInOwl:hasOBONamespace>GAZ</oboInOwl:hasOBONamespace>
        <oboInOwl:id>GAZ:00058780</oboInOwl:id>
        <rdfs:label>Mofwe Lagoon</rdfs:label>
    </owl:NamedIndividual>
    


    <!-- http://purl.obolibrary.org/obo/GAZ_00058781 -->

    <owl:NamedIndividual rdf:about="http://purl.obolibrary.org/obo/GAZ_00058781">
        <obo:IAO_0000115>A river that drains the northern Zambian plateau north of Kawambwa and flows west into the Luapula valley. It enters the Luapula swamps near the Mofwe Lagoon.</obo:IAO_0000115>
        <oboInOwl:hasOBONamespace>GAZ</oboInOwl:hasOBONamespace>
        <oboInOwl:id>GAZ:00058781</oboInOwl:id>
        <rdfs:label>Mbereshi River</rdfs:label>
    </owl:NamedIndividual>
    


    <!-- http://purl.obolibrary.org/obo/GAZ_00058782 -->

    <owl:NamedIndividual rdf:about="http://purl.obolibrary.org/obo/GAZ_00058782">
        <obo:IAO_0000115>Swamps that stretch along the last 100 km of the Luapula River before it reaches the Lake Mweru, and for much of that they are 30 km wide, covering and area of about 2500 km2. There are four inhabited islands in the DR Congo part of the delta, including the largest in the system which is connected to dry land in the dry season. Zambia has three inhabited islands in the delta including Chisenga Island. The are also many lagoons, the largest of which is Mofwe Lagoon on the Zambian side.</obo:IAO_0000115>
        <oboInOwl:hasOBONamespace>GAZ</oboInOwl:hasOBONamespace>
        <oboInOwl:id>GAZ:00058782</oboInOwl:id>
        <rdfs:label>Luapula Swamps</rdfs:label>
    </owl:NamedIndividual>
    


    <!-- http://purl.obolibrary.org/obo/GAZ_00058783 -->

    <owl:NamedIndividual rdf:about="http://purl.obolibrary.org/obo/GAZ_00058783">
        <obo:RO_0001025 rdf:resource="http://purl.obolibrary.org/obo/GAZ_00058782"/>
        <obo:IAO_0000115>A Zambian island in the Luapula Swamps.</obo:IAO_0000115>
        <oboInOwl:hasOBONamespace>GAZ</oboInOwl:hasOBONamespace>
        <oboInOwl:id>GAZ:00058783</oboInOwl:id>
        <rdfs:label>Chisenga Island</rdfs:label>
    </owl:NamedIndividual>
    


    <!-- http://purl.obolibrary.org/obo/GAZ_00058791 -->

    <owl:NamedIndividual rdf:about="http://purl.obolibrary.org/obo/GAZ_00058791">
        <obo:RO_0001025 rdf:resource="http://purl.obolibrary.org/obo/GAZ_00000007"/>
        <obo:IAO_0000115>A polymictic shallow lake complex of Uganda, about 1,720 km2 in area and at an elevation of 914 m. The Victoria Nile flows through the lake on its way from Lake Victoria to Lake Albert. The main inflow from Lake Victoria is regulated by the Nalubaale Power Station in Jinja. Another source of water is the Mount Elgon region on the border between Uganda and Kenya.</obo:IAO_0000115>
        <oboInOwl:hasOBONamespace>GAZ</oboInOwl:hasOBONamespace>
        <oboInOwl:id>GAZ:00058791</oboInOwl:id>
        <rdfs:label>Lake Kyoga</rdfs:label>
    </owl:NamedIndividual>
    


    <!-- http://purl.obolibrary.org/obo/GAZ_00058792 -->

    <owl:NamedIndividual rdf:about="http://purl.obolibrary.org/obo/GAZ_00058792">
        <obo:RO_0001025 rdf:resource="http://purl.obolibrary.org/obo/GAZ_00000007"/>
        <obo:IAO_0000115>A lake in Uganda. It drains to the SW into Lake Edward through the Kazinga Channel.</obo:IAO_0000115>
        <oboInOwl:hasOBONamespace>GAZ</oboInOwl:hasOBONamespace>
        <oboInOwl:id>GAZ:00058792</oboInOwl:id>
        <rdfs:label>Lake George</rdfs:label>
    </owl:NamedIndividual>
    


    <!-- http://purl.obolibrary.org/obo/GAZ_00058802 -->

    <owl:NamedIndividual rdf:about="http://purl.obolibrary.org/obo/GAZ_00058802">
        <obo:RO_0001025 rdf:resource="http://purl.obolibrary.org/obo/GAZ_00000007"/>
        <obo:RO_0001025 rdf:resource="http://purl.obolibrary.org/obo/GAZ_00136138"/>
        <obo:IAO_0000115>The world&apos;s largest unbroken, unflooded volcanic caldera. The Crater, which formed when a giant volcano exploded and collapsed on itself some two to three million years ago, is 610m deep and the floor is 260 km2.</obo:IAO_0000115>
        <oboInOwl:hasOBONamespace>GAZ</oboInOwl:hasOBONamespace>
        <oboInOwl:id>GAZ:00058802</oboInOwl:id>
        <rdfs:label>Ngorongoro Crater</rdfs:label>
    </owl:NamedIndividual>
    


    <!-- http://purl.obolibrary.org/obo/GAZ_00058803 -->

    <owl:NamedIndividual rdf:about="http://purl.obolibrary.org/obo/GAZ_00058803">
        <obo:RO_0001025 rdf:resource="http://purl.obolibrary.org/obo/GAZ_00000007"/>
        <obo:IAO_0000115>A steep-sided ravine in the Great Rift Valley, which stretches along eastern Africa. Olduvai is in the eastern Serengeti Plains in northern Tanzania and is about 30 miles long.</obo:IAO_0000115>
        <oboInOwl:hasOBONamespace>GAZ</oboInOwl:hasOBONamespace>
        <oboInOwl:id>GAZ:00058803</oboInOwl:id>
        <rdfs:label>Olduvai Gorge</rdfs:label>
    </owl:NamedIndividual>
    


    <!-- http://purl.obolibrary.org/obo/GAZ_00058835 -->

    <owl:NamedIndividual rdf:about="http://purl.obolibrary.org/obo/GAZ_00058835">
        <obo:RO_0001025 rdf:resource="http://purl.obolibrary.org/obo/GAZ_00058836"/>
        <obo:IAO_0000115>An oxbow lake in Kenya, at the base of the Kerio valley. The lake is 1 km2 in size. It was formed in year 1961 as a result of the Kerio River changing its course, therefore forming an oxbow lake.</obo:IAO_0000115>
        <oboInOwl:hasOBONamespace>GAZ</oboInOwl:hasOBONamespace>
        <oboInOwl:id>GAZ:00058835</oboInOwl:id>
        <rdfs:label>Lake Kamnarok</rdfs:label>
    </owl:NamedIndividual>
    


    <!-- http://purl.obolibrary.org/obo/GAZ_00058836 -->

    <owl:NamedIndividual rdf:about="http://purl.obolibrary.org/obo/GAZ_00058836">
        <obo:RO_0001025 rdf:resource="http://purl.obolibrary.org/obo/GAZ_00000007"/>
        <obo:IAO_0000115>A valley that lies between the Tugen Hills and the Elgeyo escarpment at an elevation of 1,000 m. in the Great Rift Valley in Kenya.</obo:IAO_0000115>
        <oboInOwl:hasOBONamespace>GAZ</oboInOwl:hasOBONamespace>
        <oboInOwl:id>GAZ:00058836</oboInOwl:id>
        <rdfs:label>Kerio River Valley</rdfs:label>
    </owl:NamedIndividual>
    


    <!-- http://purl.obolibrary.org/obo/GAZ_00058838 -->

    <owl:NamedIndividual rdf:about="http://purl.obolibrary.org/obo/GAZ_00058838">
        <obo:RO_0001025 rdf:resource="http://purl.obolibrary.org/obo/GAZ_00123720"/>
        <obo:IAO_0000115>An endorheic lake in the Tigray Region of Ethiopia. Located in the Ethiopian highlands at an elevation of 2,409 m.</obo:IAO_0000115>
        <oboInOwl:hasOBONamespace>GAZ</oboInOwl:hasOBONamespace>
        <oboInOwl:id>GAZ:00058838</oboInOwl:id>
        <rdfs:label>Lake Ashenge</rdfs:label>
    </owl:NamedIndividual>
    


    <!-- http://purl.obolibrary.org/obo/GAZ_00058839 -->

    <owl:NamedIndividual rdf:about="http://purl.obolibrary.org/obo/GAZ_00058839">
        <obo:RO_0001025 rdf:resource="http://purl.obolibrary.org/obo/GAZ_00123459"/>
        <obo:IAO_0000115>A freshwater lake of Ethiopia. It is located north of Dessie, in the Debub Wollo Zone of the Amhara Region. The town of Hayq is to the west of the lake.</obo:IAO_0000115>
        <oboInOwl:hasOBONamespace>GAZ</oboInOwl:hasOBONamespace>
        <oboInOwl:id>GAZ:00058839</oboInOwl:id>
        <rdfs:label>Lake Hayq</rdfs:label>
    </owl:NamedIndividual>
    


    <!-- http://purl.obolibrary.org/obo/GAZ_00058840 -->

    <owl:NamedIndividual rdf:about="http://purl.obolibrary.org/obo/GAZ_00058840">
        <obo:RO_0001025 rdf:resource="http://purl.obolibrary.org/obo/GAZ_00052554"/>
        <obo:RO_0001025 rdf:resource="http://purl.obolibrary.org/obo/GAZ_00123867"/>
        <obo:IAO_0000115>A reservoir in south-central Ethiopia. It was created by the construction of the Koka Dam across the Awash River. It is Located in the Misraq Shewa Zone of the Oromia Region. Constructed 1960.</obo:IAO_0000115>
        <oboInOwl:hasOBONamespace>GAZ</oboInOwl:hasOBONamespace>
        <oboInOwl:id>GAZ:00058840</oboInOwl:id>
        <rdfs:label>Koka Reservoir</rdfs:label>
    </owl:NamedIndividual>
    


    <!-- http://purl.obolibrary.org/obo/GAZ_00058841 -->

    <owl:NamedIndividual rdf:about="http://purl.obolibrary.org/obo/GAZ_00058841">
        <obo:RO_0001025 rdf:resource="http://purl.obolibrary.org/obo/GAZ_00123444"/>
        <obo:IAO_0000115>A crater lake located in Agew Awi Zon of Amhara Region in Ethiopia. The lake is situated between the towns Injibara and Kessa only 200 m from the Addis Ababa - Bahir Dar Highway with an elevation of 2500 m.</obo:IAO_0000115>
        <oboInOwl:hasOBONamespace>GAZ</oboInOwl:hasOBONamespace>
        <oboInOwl:id>GAZ:00058841</oboInOwl:id>
        <rdfs:label>Zengena Lake</rdfs:label>
    </owl:NamedIndividual>
    


    <!-- http://purl.obolibrary.org/obo/GAZ_00076366 -->

    <owl:NamedIndividual rdf:about="http://purl.obolibrary.org/obo/GAZ_00076366">
        <obo:RO_0001025 rdf:resource="http://purl.obolibrary.org/obo/GAZ_00000782"/>
        <obo:IAO_0000115>A proposed National Park, but the steps needed to fully protect it by the government of Ethiopia have not been completed as of 2002. Located in the Gambela Region, its 5061 km2 of territory is encroached upon by cotton plantations and refugee camps.</obo:IAO_0000115>
        <oboInOwl:hasOBONamespace>GAZ</oboInOwl:hasOBONamespace>
        <oboInOwl:id>GAZ:00076366</oboInOwl:id>
        <rdfs:label>Gambela National Park</rdfs:label>
    </owl:NamedIndividual>
    


    <!-- http://purl.obolibrary.org/obo/GAZ_00076367 -->

    <owl:NamedIndividual rdf:about="http://purl.obolibrary.org/obo/GAZ_00076367">
        <obo:RO_0001025 rdf:resource="http://purl.obolibrary.org/obo/GAZ_00123685"/>
        <obo:IAO_0000115>One of the National Parks of Ethiopia. Located in the Southern Nations, Nationalities, and Peoples Region about 782 km south of Addis Ababa, the 2162 km2 of this park are divided by the Mago River, a tributary of the Omo River, into two parts. The park office is 115 km north of Omorate and 26 km southwest of Jinka. All roads to and from the park are unpaved. The Mago National Park was established in 1979.</obo:IAO_0000115>
        <oboInOwl:hasOBONamespace>GAZ</oboInOwl:hasOBONamespace>
        <oboInOwl:id>GAZ:00076367</oboInOwl:id>
        <rdfs:label>Mago National Park</rdfs:label>
    </owl:NamedIndividual>
    


    <!-- http://purl.obolibrary.org/obo/GAZ_00076368 -->

    <owl:NamedIndividual rdf:about="http://purl.obolibrary.org/obo/GAZ_00076368">
        <obo:RO_0001025 rdf:resource="http://purl.obolibrary.org/obo/GAZ_00052578"/>
        <obo:IAO_0000115>A national parks of Ethiopia. Located in the Semien Gondar Zone of the Amhara Region, its territory covers the Semien Mountains and includes Ras Dashan, the highest point in Ethiopia and fourth-highest in Africa. Established 1969. A World Heritage Site.</obo:IAO_0000115>
        <oboInOwl:hasOBONamespace>GAZ</oboInOwl:hasOBONamespace>
        <oboInOwl:id>GAZ:00076368</oboInOwl:id>
        <rdfs:label>Semien Mountains National Park</rdfs:label>
    </owl:NamedIndividual>
    


    <!-- http://purl.obolibrary.org/obo/GAZ_00076369 -->

    <owl:NamedIndividual rdf:about="http://purl.obolibrary.org/obo/GAZ_00076369">
        <obo:RO_0001025 rdf:resource="http://purl.obolibrary.org/obo/GAZ_00031128"/>
        <obo:RO_0001025 rdf:resource="http://purl.obolibrary.org/obo/GAZ_00123417"/>
        <obo:RO_0001025 rdf:resource="http://purl.obolibrary.org/obo/GAZ_00123426"/>
        <obo:IAO_0000115>One of the National Parks of Ethiopia. Located in the Afar Region, its 4730 km2 of territory include Mount Yangudi and the surrounding Rassa Plains.</obo:IAO_0000115>
        <oboInOwl:hasOBONamespace>GAZ</oboInOwl:hasOBONamespace>
        <oboInOwl:id>GAZ:00076369</oboInOwl:id>
        <rdfs:label>Yangudi Rassa National Park</rdfs:label>
    </owl:NamedIndividual>
    


    <!-- http://purl.obolibrary.org/obo/GAZ_00076370 -->

    <owl:NamedIndividual rdf:about="http://purl.obolibrary.org/obo/GAZ_00076370">
        <obo:RO_0001025 rdf:resource="http://purl.obolibrary.org/obo/GAZ_00000567"/>
        <obo:IAO_0000115>A protected area in Ethiopia.</obo:IAO_0000115>
        <oboInOwl:hasOBONamespace>GAZ</oboInOwl:hasOBONamespace>
        <oboInOwl:id>GAZ:00076370</oboInOwl:id>
        <rdfs:label>Kuni-Muktar Mountain Nyala Sanctuary</rdfs:label>
    </owl:NamedIndividual>
    


    <!-- http://purl.obolibrary.org/obo/GAZ_00076371 -->

    <owl:NamedIndividual rdf:about="http://purl.obolibrary.org/obo/GAZ_00076371">
        <obo:RO_0001025 rdf:resource="http://purl.obolibrary.org/obo/GAZ_00000567"/>
        <obo:RO_0001025 rdf:resource="http://purl.obolibrary.org/obo/GAZ_00000786"/>
        <obo:IAO_0000115>A protected area in Ethiopia.</obo:IAO_0000115>
        <oboInOwl:hasOBONamespace>GAZ</oboInOwl:hasOBONamespace>
        <oboInOwl:id>GAZ:00076371</oboInOwl:id>
        <rdfs:label>Stephanie Wildlife Sanctuary</rdfs:label>
    </owl:NamedIndividual>
    


    <!-- http://purl.obolibrary.org/obo/GAZ_00076372 -->

    <owl:NamedIndividual rdf:about="http://purl.obolibrary.org/obo/GAZ_00076372">
        <obo:RO_0001025 rdf:resource="http://purl.obolibrary.org/obo/GAZ_00000784"/>
        <obo:IAO_0000115>A protected area in Ethiopia.</obo:IAO_0000115>
        <oboInOwl:hasOBONamespace>GAZ</oboInOwl:hasOBONamespace>
        <oboInOwl:id>GAZ:00076372</oboInOwl:id>
        <rdfs:label>Didessa Wildlife Sanctuary</rdfs:label>
    </owl:NamedIndividual>
    


    <!-- http://purl.obolibrary.org/obo/GAZ_00076373 -->

    <owl:NamedIndividual rdf:about="http://purl.obolibrary.org/obo/GAZ_00076373">
        <obo:RO_0001025 rdf:resource="http://purl.obolibrary.org/obo/GAZ_00052577"/>
        <obo:IAO_0000115>A protected area in Ethiopia. It is located in the Borena Zone of the Oromia Region, west of the town of Yabelo.</obo:IAO_0000115>
        <oboInOwl:hasOBONamespace>GAZ</oboInOwl:hasOBONamespace>
        <oboInOwl:id>GAZ:00076373</oboInOwl:id>
        <rdfs:label>Yabelo Wildlife Sanctuary</rdfs:label>
    </owl:NamedIndividual>
    


    <!-- http://purl.obolibrary.org/obo/GAZ_00076374 -->

    <owl:NamedIndividual rdf:about="http://purl.obolibrary.org/obo/GAZ_00076374">
        <obo:RO_0001025 rdf:resource="http://purl.obolibrary.org/obo/GAZ_00123903"/>
        <obo:IAO_0000115>A protected area in Ethiopia. It is located in the Misraq (East) Hararghe Zone of the Oromia Region, south of Babille.</obo:IAO_0000115>
        <oboInOwl:hasOBONamespace>GAZ</oboInOwl:hasOBONamespace>
        <oboInOwl:id>GAZ:00076374</oboInOwl:id>
        <rdfs:label>Harar Wildlife Sanctuary</rdfs:label>
    </owl:NamedIndividual>
    


    <!-- http://purl.obolibrary.org/obo/GAZ_00076375 -->

    <owl:NamedIndividual rdf:about="http://purl.obolibrary.org/obo/GAZ_00076375">
        <obo:RO_0001025 rdf:resource="http://purl.obolibrary.org/obo/GAZ_00031125"/>
        <obo:IAO_0000115>A protected area in the Oromia Region (or kilil) of Ethiopia, dedicated especially to the protection of the Swayne&apos;s Hartebeest.</obo:IAO_0000115>
        <oboInOwl:hasOBONamespace>GAZ</oboInOwl:hasOBONamespace>
        <oboInOwl:id>GAZ:00076375</oboInOwl:id>
        <rdfs:label>Senkelle Swayne&apos;s Hartebeest Sanctuary</rdfs:label>
    </owl:NamedIndividual>
    


    <!-- http://purl.obolibrary.org/obo/GAZ_00076405 -->

    <owl:NamedIndividual rdf:about="http://purl.obolibrary.org/obo/GAZ_00076405">
        <obo:RO_0001025 rdf:resource="http://purl.obolibrary.org/obo/GAZ_00000007"/>
        <obo:IAO_0000115>A national park that lies south of Lake Naivasha in Kenya, north west of Nairobi. It includes the Fischer&apos;s Tower and Central Tower columns and Hell&apos;s Gate Gorge. The national park is also home to three geothermal power stations at Olkaria.</obo:IAO_0000115>
        <oboInOwl:hasOBONamespace>GAZ</oboInOwl:hasOBONamespace>
        <oboInOwl:id>GAZ:00076405</oboInOwl:id>
        <rdfs:label>Hell&apos;s Gate National Park</rdfs:label>
    </owl:NamedIndividual>
    


    <!-- http://purl.obolibrary.org/obo/GAZ_00076707 -->

    <owl:NamedIndividual rdf:about="http://purl.obolibrary.org/obo/GAZ_00076707">
        <obo:RO_0001025 rdf:resource="http://purl.obolibrary.org/obo/GAZ_00076708"/>
        <obo:IAO_0000115>A national park in Tanzania.</obo:IAO_0000115>
        <oboInOwl:hasOBONamespace>GAZ</oboInOwl:hasOBONamespace>
        <oboInOwl:id>GAZ:00076707</oboInOwl:id>
        <rdfs:label>Rubondo Island National Park</rdfs:label>
    </owl:NamedIndividual>
    


    <!-- http://purl.obolibrary.org/obo/GAZ_00076708 -->

    <owl:NamedIndividual rdf:about="http://purl.obolibrary.org/obo/GAZ_00076708">
        <obo:RO_0001025 rdf:resource="http://purl.obolibrary.org/obo/GAZ_00015452"/>
        <obo:IAO_0000115>An island in the SW of Lake Victoria.</obo:IAO_0000115>
        <oboInOwl:hasOBONamespace>GAZ</oboInOwl:hasOBONamespace>
        <oboInOwl:id>GAZ:00076708</oboInOwl:id>
        <rdfs:label>Rubondo Island</rdfs:label>
    </owl:NamedIndividual>
    


    <!-- http://purl.obolibrary.org/obo/GAZ_00076715 -->

    <owl:NamedIndividual rdf:about="http://purl.obolibrary.org/obo/GAZ_00076715">
        <obo:RO_0001025 rdf:resource="http://purl.obolibrary.org/obo/GAZ_00000007"/>
        <obo:IAO_0000115>A protected area in Tanzania.</obo:IAO_0000115>
        <oboInOwl:hasOBONamespace>GAZ</oboInOwl:hasOBONamespace>
        <oboInOwl:id>GAZ:00076715</oboInOwl:id>
        <rdfs:label>Uwanda Game Reserve</rdfs:label>
    </owl:NamedIndividual>
    


    <!-- http://purl.obolibrary.org/obo/GAZ_00104006 -->

    <owl:NamedIndividual rdf:about="http://purl.obolibrary.org/obo/GAZ_00104006">
        <obo:RO_0001025 rdf:resource="http://purl.obolibrary.org/obo/GAZ_00031091"/>
        <oboInOwl:hasOBONamespace>GAZ</oboInOwl:hasOBONamespace>
        <oboInOwl:id>GAZ:00104006</oboInOwl:id>
        <rdfs:label>Addis Ababa Zone 2</rdfs:label>
    </owl:NamedIndividual>
    


    <!-- http://purl.obolibrary.org/obo/GAZ_00104007 -->

    <owl:NamedIndividual rdf:about="http://purl.obolibrary.org/obo/GAZ_00104007">
        <obo:RO_0001025 rdf:resource="http://purl.obolibrary.org/obo/GAZ_00031091"/>
        <oboInOwl:hasOBONamespace>GAZ</oboInOwl:hasOBONamespace>
        <oboInOwl:id>GAZ:00104007</oboInOwl:id>
        <rdfs:label>Addis Ababa Zone 5</rdfs:label>
    </owl:NamedIndividual>
    


    <!-- http://purl.obolibrary.org/obo/GAZ_00104008 -->

    <owl:NamedIndividual rdf:about="http://purl.obolibrary.org/obo/GAZ_00104008">
        <obo:RO_0001025 rdf:resource="http://purl.obolibrary.org/obo/GAZ_00031091"/>
        <oboInOwl:hasOBONamespace>GAZ</oboInOwl:hasOBONamespace>
        <oboInOwl:id>GAZ:00104008</oboInOwl:id>
        <rdfs:label>Addis Ababa Zone 4</rdfs:label>
    </owl:NamedIndividual>
    


    <!-- http://purl.obolibrary.org/obo/GAZ_00104009 -->

    <owl:NamedIndividual rdf:about="http://purl.obolibrary.org/obo/GAZ_00104009">
        <obo:RO_0001025 rdf:resource="http://purl.obolibrary.org/obo/GAZ_00031091"/>
        <oboInOwl:hasOBONamespace>GAZ</oboInOwl:hasOBONamespace>
        <oboInOwl:id>GAZ:00104009</oboInOwl:id>
        <rdfs:label>Addis Ababa Zone 3</rdfs:label>
    </owl:NamedIndividual>
    


    <!-- http://purl.obolibrary.org/obo/GAZ_00104011 -->

    <owl:NamedIndividual rdf:about="http://purl.obolibrary.org/obo/GAZ_00104011">
        <obo:RO_0001025 rdf:resource="http://purl.obolibrary.org/obo/GAZ_00031091"/>
        <oboInOwl:hasOBONamespace>GAZ</oboInOwl:hasOBONamespace>
        <oboInOwl:id>GAZ:00104011</oboInOwl:id>
        <rdfs:label>Addis Ababa Zone 6</rdfs:label>
    </owl:NamedIndividual>
    


    <!-- http://purl.obolibrary.org/obo/GAZ_00123407 -->

    <owl:NamedIndividual rdf:about="http://purl.obolibrary.org/obo/GAZ_00123407">
        <obo:RO_0001025 rdf:resource="http://purl.obolibrary.org/obo/GAZ_00031086"/>
        <obo:IAO_0000115>One of the 29 woredas in the Afar Region of Ethiopia. Part of the Administrative Zone 2, Berahle&apos;s territory includes part of the Afar Depression. This woreda is bordered on the south by Afdera and Abala, on the southwest by the Tigray Region, on the west by Koneba, on the north by Dallol, and on the northeast by Eritrea.</obo:IAO_0000115>
        <oboInOwl:hasOBONamespace>GAZ</oboInOwl:hasOBONamespace>
        <oboInOwl:id>GAZ:00123407</oboInOwl:id>
        <rdfs:label>Berahle Woreda</rdfs:label>
    </owl:NamedIndividual>
    


    <!-- http://purl.obolibrary.org/obo/GAZ_00123408 -->

    <owl:NamedIndividual rdf:about="http://purl.obolibrary.org/obo/GAZ_00123408">
        <obo:RO_0001025 rdf:resource="http://purl.obolibrary.org/obo/GAZ_00031086"/>
        <obo:IAO_0000115>One of the 29 woredas in the Afar Region of Ethiopia. Part of the Administrative Zone 2, Megale is located at the base of the eastern escarpment of the Ethiopian highlands, and bordered on the south by the Administrative Zone 4, on the west by the Tigray Region, on the north by Abala, and on the east by Erebti.</obo:IAO_0000115>
        <oboInOwl:hasOBONamespace>GAZ</oboInOwl:hasOBONamespace>
        <oboInOwl:id>GAZ:00123408</oboInOwl:id>
        <rdfs:label>Megale Woreda</rdfs:label>
    </owl:NamedIndividual>
    


    <!-- http://purl.obolibrary.org/obo/GAZ_00123409 -->

    <owl:NamedIndividual rdf:about="http://purl.obolibrary.org/obo/GAZ_00123409">
        <obo:RO_0001025 rdf:resource="http://purl.obolibrary.org/obo/GAZ_00031086"/>
        <obo:IAO_0000115>One of the 29 woredas in the Afar Region of Ethiopia. It is named after the saline Lake Afdera, located in the southern part of the Afar Depression. Part of the Administrative Zone 2, Afdera is bordered on the southwest by the Administrative Zone 4, on the west by Erebti and Abala, on the north by Berahle, on the northeast by Eritrea, and on the southeast by Administrative Zone 1.</obo:IAO_0000115>
        <oboInOwl:hasOBONamespace>GAZ</oboInOwl:hasOBONamespace>
        <oboInOwl:id>GAZ:00123409</oboInOwl:id>
        <rdfs:label>Afdera Woreda</rdfs:label>
    </owl:NamedIndividual>
    


    <!-- http://purl.obolibrary.org/obo/GAZ_00123410 -->

    <owl:NamedIndividual rdf:about="http://purl.obolibrary.org/obo/GAZ_00123410">
        <obo:RO_0001025 rdf:resource="http://purl.obolibrary.org/obo/GAZ_00031086"/>
        <obo:IAO_0000115>One of the 29 woredas in the Afar Region of Ethiopia. It is named after the Erebti River, a stream that flows east from the Ethiopian highlands into the Afar Depression, part of which lies in the eastern part of this woreda. One of the woredas in the Administrative Zone 2, Erebti is bordered on the south by the Administrative Zone 4, on the southwest by Megale, on the northwest by Abala, and on the north and east by Afdera.</obo:IAO_0000115>
        <oboInOwl:hasOBONamespace>GAZ</oboInOwl:hasOBONamespace>
        <oboInOwl:id>GAZ:00123410</oboInOwl:id>
        <rdfs:label>Erebti Woreda</rdfs:label>
    </owl:NamedIndividual>
    


    <!-- http://purl.obolibrary.org/obo/GAZ_00123411 -->

    <owl:NamedIndividual rdf:about="http://purl.obolibrary.org/obo/GAZ_00123411">
        <obo:RO_0001025 rdf:resource="http://purl.obolibrary.org/obo/GAZ_00031086"/>
        <obo:IAO_0000115>One of the 29 woredas in the Afar Region of Ethiopia. A triangle-shaped district in the Administrative Zone 2, Koneba is located near the base of the eastern escarpment of the Ethiopian highlands, and bordered on the west by the Tigray Region, on the north by Dallol, and on the east by Berahle. The major town in Koneba is Koneba.</obo:IAO_0000115>
        <oboInOwl:hasOBONamespace>GAZ</oboInOwl:hasOBONamespace>
        <oboInOwl:id>GAZ:00123411</oboInOwl:id>
        <rdfs:label>Koneba Woreda</rdfs:label>
    </owl:NamedIndividual>
    


    <!-- http://purl.obolibrary.org/obo/GAZ_00123412 -->

    <owl:NamedIndividual rdf:about="http://purl.obolibrary.org/obo/GAZ_00123412">
        <obo:RO_0001025 rdf:resource="http://purl.obolibrary.org/obo/GAZ_00031086"/>
        <obo:IAO_0000115>One of the 29 woredas in the Afar Region of Ethiopia. Part of the Administrative Zone 2, Dallol&apos;s territory includes part of the Afar Depression. This woreda is bordered on the south by Koneba, on the west by the Tigray Region, on the north by Eritrea, and on the east by Berahle.</obo:IAO_0000115>
        <oboInOwl:hasOBONamespace>GAZ</oboInOwl:hasOBONamespace>
        <oboInOwl:id>GAZ:00123412</oboInOwl:id>
        <rdfs:label>Dallol Woreda</rdfs:label>
    </owl:NamedIndividual>
    


    <!-- http://purl.obolibrary.org/obo/GAZ_00123413 -->

    <owl:NamedIndividual rdf:about="http://purl.obolibrary.org/obo/GAZ_00123413">
        <obo:RO_0001025 rdf:resource="http://purl.obolibrary.org/obo/GAZ_00031086"/>
        <obo:IAO_0000115>One of the 29 woredas in the Afar Region of Ethiopia. Part of the Administrative Zone 2, Abala is located at the base of the eastern escarpment of the Ethiopian highlands, and bordered on the south by Megale, on the west by the Tigray Region, on the north by Berahle, on the northeast by Afdera, and on the east by Erebti. The major town in Abala is Abala.</obo:IAO_0000115>
        <oboInOwl:hasOBONamespace>GAZ</oboInOwl:hasOBONamespace>
        <oboInOwl:id>GAZ:00123413</oboInOwl:id>
        <rdfs:label>Abala Woreda</rdfs:label>
    </owl:NamedIndividual>
    


    <!-- http://purl.obolibrary.org/obo/GAZ_00123414 -->

    <owl:NamedIndividual rdf:about="http://purl.obolibrary.org/obo/GAZ_00123414">
        <rdf:type rdf:resource="http://purl.obolibrary.org/obo/ENVO_00000856"/>
        <obo:RO_0001025 rdf:resource="http://purl.obolibrary.org/obo/GAZ_00123870"/>
        <obo:IAO_0000115>A populated place. A town in central Ethiopia, named after the nearby Modjo River. Located in the Misraq Shewa Zone of the Oromia Region.</obo:IAO_0000115>
        <oboInOwl:hasOBONamespace>GAZ</oboInOwl:hasOBONamespace>
        <oboInOwl:id>GAZ:00123414</oboInOwl:id>
        <rdfs:label>Mojo</rdfs:label>
    </owl:NamedIndividual>
    


    <!-- http://purl.obolibrary.org/obo/GAZ_00123415 -->

    <owl:NamedIndividual rdf:about="http://purl.obolibrary.org/obo/GAZ_00123415">
        <obo:RO_0001025 rdf:resource="http://purl.obolibrary.org/obo/GAZ_00031087"/>
        <obo:IAO_0000115>One of the 29 woredas in the Afar Region of Ethiopia. Part of the Administrative Zone 1, Asayita is bordered on the south by Afambo, on the west by Dubti, then on the north by the Awash River which separates it from Elidar, and on the east by Djibouti. The major town in Asayita is Asayita.</obo:IAO_0000115>
        <oboInOwl:hasOBONamespace>GAZ</oboInOwl:hasOBONamespace>
        <oboInOwl:id>GAZ:00123415</oboInOwl:id>
        <rdfs:label>Asayita Woreda</rdfs:label>
    </owl:NamedIndividual>
    


    <!-- http://purl.obolibrary.org/obo/GAZ_00123416 -->

    <owl:NamedIndividual rdf:about="http://purl.obolibrary.org/obo/GAZ_00123416">
        <obo:RO_0001025 rdf:resource="http://purl.obolibrary.org/obo/GAZ_00031087"/>
        <obo:IAO_0000115>One of the 29 woredas in the Afar Region of Ethiopia. Part of the Administrative Zone 1, Chifra is located near the base of the eastern escarpment of the Ethiopian highlands and bordered on the south by Mille, on the west by the Oromia Region, on the north by the Administrative Zone 4, and on the east by Dubti. The major town in Chifra is Chifra.</obo:IAO_0000115>
        <oboInOwl:hasOBONamespace>GAZ</oboInOwl:hasOBONamespace>
        <oboInOwl:id>GAZ:00123416</oboInOwl:id>
        <rdfs:label>Chifra Woreda</rdfs:label>
    </owl:NamedIndividual>
    


    <!-- http://purl.obolibrary.org/obo/GAZ_00123417 -->

    <owl:NamedIndividual rdf:about="http://purl.obolibrary.org/obo/GAZ_00123417">
        <obo:RO_0001025 rdf:resource="http://purl.obolibrary.org/obo/GAZ_00031087"/>
        <obo:IAO_0000115>One of the 29 woredas in the Afar Region of Ethiopia. It is named for the Mille River, a tributary of the Awash River, which flows through this woreda. On 2007-02-04, the Afar Regional Cabinet approved the division of this woreda, creating a new woreda out of the western part, with its administrative center to be at Hadar. Part of the Administrative Zone 1, Mille is bordered on the south by the Administrative Zone 3, on the southwest by Administrative Zone 5, on the west by the Amhara Region, on the northwest by Chifra, on the northeast by Dubti, and on the east by the Oromia Region. Towns in Mille include Mille and Eli Wuha.</obo:IAO_0000115>
        <oboInOwl:hasOBONamespace>GAZ</oboInOwl:hasOBONamespace>
        <oboInOwl:id>GAZ:00123417</oboInOwl:id>
        <rdfs:label>Mille Woreda</rdfs:label>
    </owl:NamedIndividual>
    


    <!-- http://purl.obolibrary.org/obo/GAZ_00123418 -->

    <owl:NamedIndividual rdf:about="http://purl.obolibrary.org/obo/GAZ_00123418">
        <obo:RO_0001025 rdf:resource="http://purl.obolibrary.org/obo/GAZ_00031087"/>
        <obo:IAO_0000115>One of the 29 woredas in the Afar Region of Ethiopia. On 2007-02-04, the Afar Regional Cabinet approved the division of this woreda, creating a new woreda out of the northwestern part next to Administrative Zone 2 to the border with Eritrea, centered on Biru. Part of the Administrative Zone 1, Elidar is bordered on the south by the Awash River which separates it from Asayita, on the west by Dubti, on the northwest by the Administrative Zone 2, on the northeast by Eritrea, and on the east by Djibouti. Towns in Elidar include Bure, Diche Oto, Elidar and Manda.</obo:IAO_0000115>
        <oboInOwl:hasOBONamespace>GAZ</oboInOwl:hasOBONamespace>
        <oboInOwl:id>GAZ:00123418</oboInOwl:id>
        <rdfs:label>Elidar Woreda</rdfs:label>
    </owl:NamedIndividual>
    


    <!-- http://purl.obolibrary.org/obo/GAZ_00123419 -->

    <owl:NamedIndividual rdf:about="http://purl.obolibrary.org/obo/GAZ_00123419">
        <obo:RO_0001025 rdf:resource="http://purl.obolibrary.org/obo/GAZ_00031087"/>
        <obo:IAO_0000115>One of the 29 woredas in the Afar Region of Ethiopia. On 2007-02-04, the Afar Regional Cabinet approved the division of this woreda, creating a new woreda out of the northern part, with its administrative center at Guluble Af. Part of the Administrative Zone 1, Dubti is bordered on the south by the Oromia Region, on the southwest by Mille, on the west by Chifra, on the northwest by Administrative Zone 4, on the north by the Administrative Zone 2, on the northeast by Elidar, on the east by Asayita, and on the southeast by Afambo. Towns in Dubti include Date Bahri, Dubti, Logya, Sardo and Semera.</obo:IAO_0000115>
        <oboInOwl:hasOBONamespace>GAZ</oboInOwl:hasOBONamespace>
        <oboInOwl:id>GAZ:00123419</oboInOwl:id>
        <rdfs:label>Dubti Woreda</rdfs:label>
    </owl:NamedIndividual>
    


    <!-- http://purl.obolibrary.org/obo/GAZ_00123420 -->

    <owl:NamedIndividual rdf:about="http://purl.obolibrary.org/obo/GAZ_00123420">
        <obo:RO_0001025 rdf:resource="http://purl.obolibrary.org/obo/GAZ_00031087"/>
        <obo:IAO_0000115>One of the 29 woredas in the Afar Region of Ethiopia. It is named after Lake Afambo, located at the border of this woreda with Asayita, near the international border with Djibouti. Part of the Administrative Zone 1, Afambo is bordered on the south by the Oromia Region, on the west by Dubti, on the north by Asayita, and on the east by Djibouti.</obo:IAO_0000115>
        <oboInOwl:hasOBONamespace>GAZ</oboInOwl:hasOBONamespace>
        <oboInOwl:id>GAZ:00123420</oboInOwl:id>
        <rdfs:label>Afambo Woreda</rdfs:label>
    </owl:NamedIndividual>
    


    <!-- http://purl.obolibrary.org/obo/GAZ_00123421 -->

    <owl:NamedIndividual rdf:about="http://purl.obolibrary.org/obo/GAZ_00123421">
        <obo:RO_0001025 rdf:resource="http://purl.obolibrary.org/obo/GAZ_00123420"/>
        <obo:IAO_0000115>A lake.</obo:IAO_0000115>
        <oboInOwl:hasOBONamespace>GAZ</oboInOwl:hasOBONamespace>
        <oboInOwl:id>GAZ:00123421</oboInOwl:id>
        <rdfs:label>Lake Laitali</rdfs:label>
    </owl:NamedIndividual>
    


    <!-- http://purl.obolibrary.org/obo/GAZ_00123422 -->

    <owl:NamedIndividual rdf:about="http://purl.obolibrary.org/obo/GAZ_00123422">
        <obo:RO_0001025 rdf:resource="http://purl.obolibrary.org/obo/GAZ_00123420"/>
        <obo:IAO_0000115>A lake.</obo:IAO_0000115>
        <oboInOwl:hasOBONamespace>GAZ</oboInOwl:hasOBONamespace>
        <oboInOwl:id>GAZ:00123422</oboInOwl:id>
        <rdfs:label>Lake Bario</rdfs:label>
    </owl:NamedIndividual>
    


    <!-- http://purl.obolibrary.org/obo/GAZ_00123423 -->

    <owl:NamedIndividual rdf:about="http://purl.obolibrary.org/obo/GAZ_00123423">
        <obo:RO_0001025 rdf:resource="http://purl.obolibrary.org/obo/GAZ_00123420"/>
        <obo:IAO_0000115>A lake.</obo:IAO_0000115>
        <oboInOwl:hasOBONamespace>GAZ</oboInOwl:hasOBONamespace>
        <oboInOwl:id>GAZ:00123423</oboInOwl:id>
        <rdfs:label>Lake Gummare</rdfs:label>
    </owl:NamedIndividual>
    


    <!-- http://purl.obolibrary.org/obo/GAZ_00123424 -->

    <owl:NamedIndividual rdf:about="http://purl.obolibrary.org/obo/GAZ_00123424">
        <obo:RO_0001025 rdf:resource="http://purl.obolibrary.org/obo/GAZ_00123420"/>
        <obo:IAO_0000115>A lake.</obo:IAO_0000115>
        <oboInOwl:hasOBONamespace>GAZ</oboInOwl:hasOBONamespace>
        <oboInOwl:id>GAZ:00123424</oboInOwl:id>
        <rdfs:label>Lake Afambo</rdfs:label>
    </owl:NamedIndividual>
    


    <!-- http://purl.obolibrary.org/obo/GAZ_00123425 -->

    <owl:NamedIndividual rdf:about="http://purl.obolibrary.org/obo/GAZ_00123425">
        <obo:RO_0001025 rdf:resource="http://purl.obolibrary.org/obo/GAZ_00031089"/>
        <obo:IAO_0000115>One of the 29 woredas in the Afar Region of Ethiopia. Part of the Administrative Zone 3, Amibara is bordered on the south by Awash Fentale, on the west by the Awash River which separates it from Dulecha to the southwest then on the northwest by the Administrative Zone 5, on the north by Gewane, and on the east by the Oromia Region. Towns in Amibara include Awash Arba, Awash Sheleko, Melka Sedi and Melka Werer.</obo:IAO_0000115>
        <oboInOwl:hasOBONamespace>GAZ</oboInOwl:hasOBONamespace>
        <oboInOwl:id>GAZ:00123425</oboInOwl:id>
        <rdfs:label>Amibara Woreda</rdfs:label>
    </owl:NamedIndividual>
    


    <!-- http://purl.obolibrary.org/obo/GAZ_00123426 -->

    <owl:NamedIndividual rdf:about="http://purl.obolibrary.org/obo/GAZ_00123426">
        <obo:RO_0001025 rdf:resource="http://purl.obolibrary.org/obo/GAZ_00031089"/>
        <obo:IAO_0000115>One of the 29 woredas in the Afar Region of Ethiopia. Part of the Administrative Zone 3, Gewane is bordered on the south by Amibara, on the west by Bure Mudaytu, on the northwest by Administrative Zone 5, on the north by the Administrative Zone 1, on the east by the Somali Region, and on the southeast by the Oromia Region; the Awash River defines parts of the boundary with Administrative Zones 3 and 5. Towns in Gewane include Meteka and Gewane.</obo:IAO_0000115>
        <oboInOwl:hasOBONamespace>GAZ</oboInOwl:hasOBONamespace>
        <oboInOwl:id>GAZ:00123426</oboInOwl:id>
        <rdfs:label>Gewane Woreda</rdfs:label>
    </owl:NamedIndividual>
    


    <!-- http://purl.obolibrary.org/obo/GAZ_00123427 -->

    <owl:NamedIndividual rdf:about="http://purl.obolibrary.org/obo/GAZ_00123427">
        <obo:RO_0001025 rdf:resource="http://purl.obolibrary.org/obo/GAZ_00031089"/>
        <obo:IAO_0000115>One of the 29 woredas in the Afar Region of Ethiopia. Part of the Administrative Zone 3, Awash Fentale is bordered on the south by the Oromia Region, on the west by the Amhara Region, on the north by Dulecha, and on the east by Amibara. Towns in Awash Fentale include Awash Sebat Kilo and Sabure.</obo:IAO_0000115>
        <oboInOwl:hasOBONamespace>GAZ</oboInOwl:hasOBONamespace>
        <oboInOwl:id>GAZ:00123427</oboInOwl:id>
        <rdfs:label>Awash Fentale Woreda</rdfs:label>
    </owl:NamedIndividual>
    


    <!-- http://purl.obolibrary.org/obo/GAZ_00123428 -->

    <owl:NamedIndividual rdf:about="http://purl.obolibrary.org/obo/GAZ_00123428">
        <obo:RO_0001025 rdf:resource="http://purl.obolibrary.org/obo/GAZ_00031089"/>
        <obo:IAO_0000115>One of the 29 woredas in the Afar Region of Ethiopia. Part of the Administrative Zone 3, Dulecha is bordered on the south by Awash Fentale, on the west by the Argobba special woreda, on the north by the Administrative Zone 5, and on the east by the Awash River which separates it from Amibara. The largest settlement in Dulecha is Dulecha.</obo:IAO_0000115>
        <oboInOwl:hasOBONamespace>GAZ</oboInOwl:hasOBONamespace>
        <oboInOwl:id>GAZ:00123428</oboInOwl:id>
        <rdfs:label>Dulecha Woreda</rdfs:label>
    </owl:NamedIndividual>
    


    <!-- http://purl.obolibrary.org/obo/GAZ_00123429 -->

    <owl:NamedIndividual rdf:about="http://purl.obolibrary.org/obo/GAZ_00123429">
        <obo:RO_0001025 rdf:resource="http://purl.obolibrary.org/obo/GAZ_00031089"/>
        <obo:IAO_0000115>One of the 29 woredas in the Afar Region of Ethiopia. Part of the Administrative Zone 3, Bure Mudaytu stretches in a narrow band between the Awash River (which separates it from the Administrative Zone 5) to the west and Gewane to the east. Information is lacking on the towns of this woreda.</obo:IAO_0000115>
        <oboInOwl:hasOBONamespace>GAZ</oboInOwl:hasOBONamespace>
        <oboInOwl:id>GAZ:00123429</oboInOwl:id>
        <rdfs:label>Bure Mudaytu Woreda</rdfs:label>
    </owl:NamedIndividual>
    


    <!-- http://purl.obolibrary.org/obo/GAZ_00123430 -->

    <owl:NamedIndividual rdf:about="http://purl.obolibrary.org/obo/GAZ_00123430">
        <obo:RO_0001025 rdf:resource="http://purl.obolibrary.org/obo/GAZ_00123429"/>
        <obo:IAO_0000115>A lake.</obo:IAO_0000115>
        <oboInOwl:hasOBONamespace>GAZ</oboInOwl:hasOBONamespace>
        <oboInOwl:id>GAZ:00123430</oboInOwl:id>
        <rdfs:label>Lake Yardi</rdfs:label>
    </owl:NamedIndividual>
    


    <!-- http://purl.obolibrary.org/obo/GAZ_00123431 -->

    <owl:NamedIndividual rdf:about="http://purl.obolibrary.org/obo/GAZ_00123431">
        <obo:RO_0001025 rdf:resource="http://purl.obolibrary.org/obo/GAZ_00031088"/>
        <obo:IAO_0000115>One of the 29 woredas in the Afar Region of Ethiopia. Part of the Administrative Zone 4, Aura is bordered on the southwest by Ewa, on the west by Gulina, on the north by Teru, and on the east by Administrative Zone 1. The largest settlement in Aura is Derayitu.</obo:IAO_0000115>
        <oboInOwl:hasOBONamespace>GAZ</oboInOwl:hasOBONamespace>
        <oboInOwl:id>GAZ:00123431</oboInOwl:id>
        <rdfs:label>Aura Woreda</rdfs:label>
    </owl:NamedIndividual>
    


    <!-- http://purl.obolibrary.org/obo/GAZ_00123432 -->

    <owl:NamedIndividual rdf:about="http://purl.obolibrary.org/obo/GAZ_00123432">
        <obo:RO_0001025 rdf:resource="http://purl.obolibrary.org/obo/GAZ_00031088"/>
        <obo:IAO_0000115>One of the 29 woredas in the Afar Region of Ethiopia. Part of the Administrative Zone 4, Ewa is located near the base of the eastern escarpment of the Ethiopian highlands, and bordered on the south by the Administrative Zone 1, on the west by the Amhara Region, on the north by Gulina, and on the east by Aura. The major settlement in Ewa is Alele Subula.</obo:IAO_0000115>
        <oboInOwl:hasOBONamespace>GAZ</oboInOwl:hasOBONamespace>
        <oboInOwl:id>GAZ:00123432</oboInOwl:id>
        <rdfs:label>Ewa Woreda</rdfs:label>
    </owl:NamedIndividual>
    


    <!-- http://purl.obolibrary.org/obo/GAZ_00123433 -->

    <owl:NamedIndividual rdf:about="http://purl.obolibrary.org/obo/GAZ_00123433">
        <obo:RO_0001025 rdf:resource="http://purl.obolibrary.org/obo/GAZ_00031088"/>
        <obo:IAO_0000115>One of the 29 woredas in the Afar Region of Ethiopia. Part of the Administrative Zone 4, Yalo is located at the base of the eastern escarpment of the Ethiopian highlands, and bordered on the south by Gulina, on the west by the Amhara Region, on the north by the Administrative Zone 2, and on the east by Teru. The major town in Yalo is Dibina.</obo:IAO_0000115>
        <oboInOwl:hasOBONamespace>GAZ</oboInOwl:hasOBONamespace>
        <oboInOwl:id>GAZ:00123433</oboInOwl:id>
        <rdfs:label>Yalo Woreda</rdfs:label>
    </owl:NamedIndividual>
    


    <!-- http://purl.obolibrary.org/obo/GAZ_00123434 -->

    <owl:NamedIndividual rdf:about="http://purl.obolibrary.org/obo/GAZ_00123434">
        <obo:RO_0001025 rdf:resource="http://purl.obolibrary.org/obo/GAZ_00031088"/>
        <obo:IAO_0000115>One of the 29 woredas in the Afar Region of Ethiopia. Part of the Administrative Zone 4, Gulina is located near the base of the eastern escarpment of the Ethiopian highlands, and bordered on the south by Ewa, on the west by the Amhara Region, on the north by Yalo, and on the east by Aura. The major settlement in Gulina is Kelewina.</obo:IAO_0000115>
        <oboInOwl:hasOBONamespace>GAZ</oboInOwl:hasOBONamespace>
        <oboInOwl:id>GAZ:00123434</oboInOwl:id>
        <rdfs:label>Gulina Woreda</rdfs:label>
    </owl:NamedIndividual>
    


    <!-- http://purl.obolibrary.org/obo/GAZ_00123435 -->

    <owl:NamedIndividual rdf:about="http://purl.obolibrary.org/obo/GAZ_00123435">
        <obo:RO_0001025 rdf:resource="http://purl.obolibrary.org/obo/GAZ_00031088"/>
        <obo:IAO_0000115>One of the 29 woredas in the Afar Region of Ethiopia. Part of the Administrative Zone 4, Teru is bordered on the south by Aura, on the southwest by Gulina, on the west by Yalo, and on the north and east by the Administrative Zone 2. Information is lacking on the towns of this woreda.</obo:IAO_0000115>
        <oboInOwl:hasOBONamespace>GAZ</oboInOwl:hasOBONamespace>
        <oboInOwl:id>GAZ:00123435</oboInOwl:id>
        <rdfs:label>Teru Woreda</rdfs:label>
    </owl:NamedIndividual>
    


    <!-- http://purl.obolibrary.org/obo/GAZ_00123436 -->

    <owl:NamedIndividual rdf:about="http://purl.obolibrary.org/obo/GAZ_00123436">
        <obo:RO_0001025 rdf:resource="http://purl.obolibrary.org/obo/GAZ_00031090"/>
        <obo:IAO_0000115>One of the 29 woredas in the Afar Region of Ethiopia. Part of the Administrative Zone 5, Artuma is a triangle-shaped district located near the base of the eastern escarpment of the Ethiopian highlands, and bordered on the south by Fursi, on the west by the Amhara Region, and on the north by Dewe.</obo:IAO_0000115>
        <oboInOwl:hasOBONamespace>GAZ</oboInOwl:hasOBONamespace>
        <oboInOwl:id>GAZ:00123436</oboInOwl:id>
        <rdfs:label>Artuma Woreda</rdfs:label>
    </owl:NamedIndividual>
    


    <!-- http://purl.obolibrary.org/obo/GAZ_00123437 -->

    <owl:NamedIndividual rdf:about="http://purl.obolibrary.org/obo/GAZ_00123437">
        <obo:RO_0001025 rdf:resource="http://purl.obolibrary.org/obo/GAZ_00031090"/>
        <obo:IAO_0000115>One of the 29 woredas in the Afar Region of Ethiopia. Part of the Administrative Zone 5.</obo:IAO_0000115>
        <oboInOwl:hasOBONamespace>GAZ</oboInOwl:hasOBONamespace>
        <oboInOwl:id>GAZ:00123437</oboInOwl:id>
        <rdfs:label>Furse Woreda</rdfs:label>
    </owl:NamedIndividual>
    


    <!-- http://purl.obolibrary.org/obo/GAZ_00123438 -->

    <owl:NamedIndividual rdf:about="http://purl.obolibrary.org/obo/GAZ_00123438">
        <obo:RO_0001025 rdf:resource="http://purl.obolibrary.org/obo/GAZ_00031090"/>
        <obo:IAO_0000115>One of the 29 woredas in the Afar Region of Ethiopia. Part of the Administrative Zone 5, Telalak is located near the base of the eastern escarpment of the Ethiopian highlands, and bordered on the south by Dewe, on the west by the Amhara Region, on the north by the Administrative Zone 4, and on the east by the Administrative Zone 3.</obo:IAO_0000115>
        <oboInOwl:hasOBONamespace>GAZ</oboInOwl:hasOBONamespace>
        <oboInOwl:id>GAZ:00123438</oboInOwl:id>
        <rdfs:label>Telalak Woreda</rdfs:label>
    </owl:NamedIndividual>
    


    <!-- http://purl.obolibrary.org/obo/GAZ_00123439 -->

    <owl:NamedIndividual rdf:about="http://purl.obolibrary.org/obo/GAZ_00123439">
        <obo:RO_0001025 rdf:resource="http://purl.obolibrary.org/obo/GAZ_00031090"/>
        <obo:IAO_0000115>One of the 29 woredas in the Afar Region of Ethiopia. Part of the Administrative Zone 5, Simurobi Gele&apos;alo is located near the base of the eastern escarpment of the Ethiopian highlands, and bordered on the west by the Amhara Region, on the north by Fursi, and on the east and south by the Administrative Zone 3; the Awash River defines the eastern boundary of this woreda with Administrative Zone 3.</obo:IAO_0000115>
        <oboInOwl:hasOBONamespace>GAZ</oboInOwl:hasOBONamespace>
        <oboInOwl:id>GAZ:00123439</oboInOwl:id>
        <rdfs:label>Simurobi Woreda</rdfs:label>
    </owl:NamedIndividual>
    


    <!-- http://purl.obolibrary.org/obo/GAZ_00123440 -->

    <owl:NamedIndividual rdf:about="http://purl.obolibrary.org/obo/GAZ_00123440">
        <obo:RO_0001025 rdf:resource="http://purl.obolibrary.org/obo/GAZ_00031090"/>
        <obo:IAO_0000115>One of the 29 woredas in the Afar Region of Ethiopia. Part of the Administrative Zone 5, Dewe is located near the base of the eastern escarpment of the Ethiopian highlands, and bordered on the south by Artuma, on the west by the Amhara Region, on the north by the Administrative Zone 4, and on the east by the Awash River which separates it from Administrative Zone 3. Information is lacking on the towns and cities of this woreda.</obo:IAO_0000115>
        <oboInOwl:hasOBONamespace>GAZ</oboInOwl:hasOBONamespace>
        <oboInOwl:id>GAZ:00123440</oboInOwl:id>
        <rdfs:label>Dewe Woreda</rdfs:label>
    </owl:NamedIndividual>
    


    <!-- http://purl.obolibrary.org/obo/GAZ_00123441 -->

    <owl:NamedIndividual rdf:about="http://purl.obolibrary.org/obo/GAZ_00123441">
        <obo:RO_0001025 rdf:resource="http://purl.obolibrary.org/obo/GAZ_00031098"/>
        <obo:IAO_0000115>One of the 105 woredas in the Amhara Region of Ethiopia. A triangle-shaped district in the Agew Awi Zone, Ankesha is bordered on the south by the Mirab Gojjam Zone, on the west by Guangua, and on the north by Banja. Towns in Ankesha include Agew Gimjabet and Azena.</obo:IAO_0000115>
        <oboInOwl:hasOBONamespace>GAZ</oboInOwl:hasOBONamespace>
        <oboInOwl:id>GAZ:00123441</oboInOwl:id>
        <rdfs:label>Ankesha Woreda</rdfs:label>
    </owl:NamedIndividual>
    


    <!-- http://purl.obolibrary.org/obo/GAZ_00123442 -->

    <owl:NamedIndividual rdf:about="http://purl.obolibrary.org/obo/GAZ_00123442">
        <obo:RO_0001025 rdf:resource="http://purl.obolibrary.org/obo/GAZ_00031098"/>
        <obo:IAO_0000115>One of the 105 woredas in the Amhara Region of Ethiopia. Part of the Agew Awi Zone, Faggeta Lekoma is bordered on the south by Banja, on the west by Guangua, on the north by Dangila, and on the east by the Mirab Gojjam Zone. Towns in Faggeta Lekoma include Addis Kidame and Faggeta.</obo:IAO_0000115>
        <oboInOwl:hasOBONamespace>GAZ</oboInOwl:hasOBONamespace>
        <oboInOwl:id>GAZ:00123442</oboInOwl:id>
        <rdfs:label>Faggeta Lekoma Woreda</rdfs:label>
    </owl:NamedIndividual>
    


    <!-- http://purl.obolibrary.org/obo/GAZ_00123443 -->

    <owl:NamedIndividual rdf:about="http://purl.obolibrary.org/obo/GAZ_00123443">
        <obo:RO_0001025 rdf:resource="http://purl.obolibrary.org/obo/GAZ_00031098"/>
        <obo:IAO_0000115>One of the 105 woredas in the Amhara Region of Ethiopia. Part of the Agew Awi Zone, Dangila is bordered on the south by Faggeta Lekoma, on the southwest by Guangua, on the west by the Benishangul-Gumuz Region, on the northwest by the Semien Gondar Zone, and on the north and east by the Mirab Gojjam Zone. Towns in Dangila include Addis Alem, Dangila and Dek.</obo:IAO_0000115>
        <oboInOwl:hasOBONamespace>GAZ</oboInOwl:hasOBONamespace>
        <oboInOwl:id>GAZ:00123443</oboInOwl:id>
        <rdfs:label>Dangila Woreda</rdfs:label>
    </owl:NamedIndividual>
    


    <!-- http://purl.obolibrary.org/obo/GAZ_00123444 -->

    <owl:NamedIndividual rdf:about="http://purl.obolibrary.org/obo/GAZ_00123444">
        <obo:RO_0001025 rdf:resource="http://purl.obolibrary.org/obo/GAZ_00031098"/>
        <obo:IAO_0000115>One of the 105 woredas in the Amhara Region of Ethiopia. Part of the Agew Awi Zone, Banja is bordered on the south by Ankesha, on the west by Guangua, on the north by Faggeta Lekoma, and on the east by the Mirab Gojjam Zone. Towns in Banja include Injibara, Kessa, Kosober and Tilili. It is also the location of the Zengena crater lake.</obo:IAO_0000115>
        <oboInOwl:hasOBONamespace>GAZ</oboInOwl:hasOBONamespace>
        <oboInOwl:id>GAZ:00123444</oboInOwl:id>
        <rdfs:label>Banja Woreda</rdfs:label>
    </owl:NamedIndividual>
    


    <!-- http://purl.obolibrary.org/obo/GAZ_00123445 -->

    <owl:NamedIndividual rdf:about="http://purl.obolibrary.org/obo/GAZ_00123445">
        <obo:RO_0001025 rdf:resource="http://purl.obolibrary.org/obo/GAZ_00031098"/>
        <obo:IAO_0000115>One of the 105 woredas in the Amhara Region of Ethiopia. Part of the Agew Awi Zone, Guangua is bordered on the south by the Abay River, which separates it from the Oromia Region, on the west by the Benishangul-Gumuz Region, on the north by Dangila, on the northwest by Faggeta Lekoma, and on the east by Ankesha. Towns in Guangua include Chagni, Kilaj, and Menta Wuha.</obo:IAO_0000115>
        <oboInOwl:hasOBONamespace>GAZ</oboInOwl:hasOBONamespace>
        <oboInOwl:id>GAZ:00123445</oboInOwl:id>
        <rdfs:label>Guangua Woreda</rdfs:label>
    </owl:NamedIndividual>
    


    <!-- http://purl.obolibrary.org/obo/GAZ_00123446 -->

    <owl:NamedIndividual rdf:about="http://purl.obolibrary.org/obo/GAZ_00123446">
        <obo:RO_0001025 rdf:resource="http://purl.obolibrary.org/obo/GAZ_00031102"/>
        <obo:IAO_0000115>One of the 105 woredas in the Amhara Region of Ethiopia. Part of the Debub Gondar Zone, Kemekem is bordered on the south by Fogera, on the west by Lake Tana, on the north by the Semien Gondar Zone, and on the east by Ebenat. The administrative center is Addis Zemen; other towns include Amba Meda, Wereta and Yifag.</obo:IAO_0000115>
        <oboInOwl:hasOBONamespace>GAZ</oboInOwl:hasOBONamespace>
        <oboInOwl:id>GAZ:00123446</oboInOwl:id>
        <rdfs:label>Kemekem Woreda</rdfs:label>
    </owl:NamedIndividual>
    


    <!-- http://purl.obolibrary.org/obo/GAZ_00123447 -->

    <owl:NamedIndividual rdf:about="http://purl.obolibrary.org/obo/GAZ_00123447">
        <obo:RO_0001025 rdf:resource="http://purl.obolibrary.org/obo/GAZ_00031102"/>
        <obo:IAO_0000115>One of the 105 woredas in the Amhara Region of Ethiopia. Part of the Debub Gondar Zone, Simada is bordered on the southeast by the Bashilo River which separates it from the Debub Wollo Zone, on the southwest by the Abbay River which separates it from the Misraq Gojjam Zone, on the northwest by Este, and on the east by Tach Gayint. The major town in Simada is Wegeda.</obo:IAO_0000115>
        <oboInOwl:hasOBONamespace>GAZ</oboInOwl:hasOBONamespace>
        <oboInOwl:id>GAZ:00123447</oboInOwl:id>
        <rdfs:label>Simada Woreda</rdfs:label>
    </owl:NamedIndividual>
    


    <!-- http://purl.obolibrary.org/obo/GAZ_00123448 -->

    <owl:NamedIndividual rdf:about="http://purl.obolibrary.org/obo/GAZ_00123448">
        <obo:RO_0001025 rdf:resource="http://purl.obolibrary.org/obo/GAZ_00031102"/>
        <obo:IAO_0000115>One of the 105 woredas in the Amhara Region of Ethiopia. Part of the Debub Gondar Zone, Tach Gayint is bordered on the south by the Bashilo River which separates it from the Debub Wollo Zone, on the west by Simada, on the north by Lay Gayint, and on the east by the Wag Hemra Zone. The major town in Tach Gayint is Arb Gebeya.</obo:IAO_0000115>
        <oboInOwl:hasOBONamespace>GAZ</oboInOwl:hasOBONamespace>
        <oboInOwl:id>GAZ:00123448</oboInOwl:id>
        <rdfs:label>Tach Gayint Woreda</rdfs:label>
    </owl:NamedIndividual>
    


    <!-- http://purl.obolibrary.org/obo/GAZ_00123449 -->

    <owl:NamedIndividual rdf:about="http://purl.obolibrary.org/obo/GAZ_00123449">
        <obo:RO_0001025 rdf:resource="http://purl.obolibrary.org/obo/GAZ_00031102"/>
        <obo:IAO_0000115>A woreda in north-central Ethiopia. Located in the Debub Gondar Zone of the Amhara Region of Ethiopia, about 100 km southeast of Gondar and 50 km east of Lake Tana.</obo:IAO_0000115>
        <oboInOwl:hasOBONamespace>GAZ</oboInOwl:hasOBONamespace>
        <oboInOwl:id>GAZ:00123449</oboInOwl:id>
        <rdfs:label>Debre Tabor Woreda</rdfs:label>
    </owl:NamedIndividual>
    


    <!-- http://purl.obolibrary.org/obo/GAZ_00123450 -->

    <owl:NamedIndividual rdf:about="http://purl.obolibrary.org/obo/GAZ_00123450">
        <obo:RO_0001025 rdf:resource="http://purl.obolibrary.org/obo/GAZ_00031102"/>
        <obo:IAO_0000115>One of the 105 woredas in the Amhara Region of Ethiopia. Part of the Debub Gondar Zone, Farta is bordered on the south by Este, on the west by Fogera, on the north by Ebenat, and on the east by Lay Gayint. Towns and cities in Farta include Gasay and Kimir Dingay.</obo:IAO_0000115>
        <oboInOwl:hasOBONamespace>GAZ</oboInOwl:hasOBONamespace>
        <oboInOwl:id>GAZ:00123450</oboInOwl:id>
        <rdfs:label>Farta Woreda</rdfs:label>
    </owl:NamedIndividual>
    


    <!-- http://purl.obolibrary.org/obo/GAZ_00123451 -->

    <owl:NamedIndividual rdf:about="http://purl.obolibrary.org/obo/GAZ_00123451">
        <obo:RO_0001025 rdf:resource="http://purl.obolibrary.org/obo/GAZ_00031102"/>
        <obo:IAO_0000115>One of the 105 woredas in the Amhara Region of Ethiopia. Part of the Debub Gondar Zone, Ebenat is bordered on the south by Farta, on the west by Kemekem, on the northwest by the Semien Gondar Zone, on the northeast by the Wag Hemra Zone, and on the east by Lay Gayint. The administrative center of Ebenat is Ebenat.</obo:IAO_0000115>
        <oboInOwl:hasOBONamespace>GAZ</oboInOwl:hasOBONamespace>
        <oboInOwl:id>GAZ:00123451</oboInOwl:id>
        <rdfs:label>Ebenat Woreda</rdfs:label>
    </owl:NamedIndividual>
    


    <!-- http://purl.obolibrary.org/obo/GAZ_00123452 -->

    <owl:NamedIndividual rdf:about="http://purl.obolibrary.org/obo/GAZ_00123452">
        <obo:RO_0001025 rdf:resource="http://purl.obolibrary.org/obo/GAZ_00031102"/>
        <obo:IAO_0000115>One of the 105 woredas in the Amhara Region of Ethiopia. Part of the Debub Gondar Zone, Dera is bordered on the south by the Abbay River which separates it from the Misraq Gojjam Zone, on the west by Lake Tana, on the north by Fogera, and on the east by Este. Towns in Dera include Amba Same, Arb Gebeya and Hamusit.</obo:IAO_0000115>
        <oboInOwl:hasOBONamespace>GAZ</oboInOwl:hasOBONamespace>
        <oboInOwl:id>GAZ:00123452</oboInOwl:id>
        <rdfs:label>Dera Woreda</rdfs:label>
    </owl:NamedIndividual>
    


    <!-- http://purl.obolibrary.org/obo/GAZ_00123453 -->

    <owl:NamedIndividual rdf:about="http://purl.obolibrary.org/obo/GAZ_00123453">
        <obo:RO_0001025 rdf:resource="http://purl.obolibrary.org/obo/GAZ_00031102"/>
        <obo:IAO_0000115>One of the 105 woredas in the Amhara Region of Ethiopia. Part of the Debub Gondar Zone, Lay Gayint is bordered on the south by Tach Gayint, on the southwest by Este, on the west by Farta, on the north by Ebenat, and on the east by the Wag Hemra Zone. Towns in Lay Gayint include Gobgob, Nefas Mewcha and Sali.</obo:IAO_0000115>
        <oboInOwl:hasOBONamespace>GAZ</oboInOwl:hasOBONamespace>
        <oboInOwl:id>GAZ:00123453</oboInOwl:id>
        <rdfs:label>Lay Gayint Woreda</rdfs:label>
    </owl:NamedIndividual>
    


    <!-- http://purl.obolibrary.org/obo/GAZ_00123454 -->

    <owl:NamedIndividual rdf:about="http://purl.obolibrary.org/obo/GAZ_00123454">
        <obo:RO_0001025 rdf:resource="http://purl.obolibrary.org/obo/GAZ_00031102"/>
        <obo:IAO_0000115>One of the 105 woredas in the Amhara Region of Ethiopia. Part of the Debub Gondar Zone, Fogera is bordered on the south by Dera, on the west by Lake Tana, on the north by Kemekem, and on the east by Farta. The major town in Fogera is Amed Ber.</obo:IAO_0000115>
        <oboInOwl:hasOBONamespace>GAZ</oboInOwl:hasOBONamespace>
        <oboInOwl:id>GAZ:00123454</oboInOwl:id>
        <rdfs:label>Fogera Woreda</rdfs:label>
    </owl:NamedIndividual>
    


    <!-- http://purl.obolibrary.org/obo/GAZ_00123455 -->

    <owl:NamedIndividual rdf:about="http://purl.obolibrary.org/obo/GAZ_00123455">
        <obo:RO_0001025 rdf:resource="http://purl.obolibrary.org/obo/GAZ_00031102"/>
        <obo:IAO_0000115>One of the 105 woredas in the Amhara Region of Ethiopia. Part of the Debub Gondar Zone, Este is bordered on the south by the Abay River which separates it from the Misraq Gojjam Zone, on the west by Dera, on the northwest by Fogera, on the north by Farta, on the northeast by Lay Gayint, and on the east by Simada. Towns in Este include Jara Gedo and Mekane Yesus.</obo:IAO_0000115>
        <oboInOwl:hasOBONamespace>GAZ</oboInOwl:hasOBONamespace>
        <oboInOwl:id>GAZ:00123455</oboInOwl:id>
        <rdfs:label>Este Woreda</rdfs:label>
    </owl:NamedIndividual>
    


    <!-- http://purl.obolibrary.org/obo/GAZ_00123456 -->

    <owl:NamedIndividual rdf:about="http://purl.obolibrary.org/obo/GAZ_00123456">
        <obo:RO_0001025 rdf:resource="http://purl.obolibrary.org/obo/GAZ_00031094"/>
        <obo:IAO_0000115>One of the 105 woredas in the Amhara Region of Ethiopia. Part of the Debub Wollo Zone, Debre Sina is bordered on the south by Wegde, on the west by the Abbay River which separates it from the Misraq Gojjam Zone, on the north by Sayint, and on the east by Legambo. Towns in Debre Sina include Amsale Genet and Mekane Selam.</obo:IAO_0000115>
        <oboInOwl:hasOBONamespace>GAZ</oboInOwl:hasOBONamespace>
        <oboInOwl:id>GAZ:00123456</oboInOwl:id>
        <rdfs:label>Debre Sina Woreda</rdfs:label>
    </owl:NamedIndividual>
    


    <!-- http://purl.obolibrary.org/obo/GAZ_00123457 -->

    <owl:NamedIndividual rdf:about="http://purl.obolibrary.org/obo/GAZ_00123457">
        <obo:RO_0001025 rdf:resource="http://purl.obolibrary.org/obo/GAZ_00031094"/>
        <obo:IAO_0000115>One of the 105 woredas in the Amhara Region of Ethiopia. Part of the Debub Wollo Zone, Were Ilu is bordered on the southwest by Jama, on the west by Kelala, on the northwest by Legambo, on the north by the Dessie Zuria, on the east by the Oromia Zone, and on the southeast by Semien Shewa Zone. Towns in Were Ilu include Kabe, Were Ilu and Weyin Amba.</obo:IAO_0000115>
        <oboInOwl:hasOBONamespace>GAZ</oboInOwl:hasOBONamespace>
        <oboInOwl:id>GAZ:00123457</oboInOwl:id>
        <rdfs:label>Were Ilu Woreda</rdfs:label>
    </owl:NamedIndividual>
    


    <!-- http://purl.obolibrary.org/obo/GAZ_00123458 -->

    <owl:NamedIndividual rdf:about="http://purl.obolibrary.org/obo/GAZ_00123458">
        <obo:RO_0001025 rdf:resource="http://purl.obolibrary.org/obo/GAZ_00031094"/>
        <obo:IAO_0000115>One of the 105 woredas in the Amhara Region of Ethiopia. Part of the Debub Wollo Zone, Wegde is bordered on the south by the Walaqa River which separates it from the Oromia Region, on the west by the Abay River which separates it from the Misraq Gojjam Zone, on the north by Debre Sina, and on the east by Kelala. The major town in Wegde is Mahdere Selam.</obo:IAO_0000115>
        <oboInOwl:hasOBONamespace>GAZ</oboInOwl:hasOBONamespace>
        <oboInOwl:id>GAZ:00123458</oboInOwl:id>
        <rdfs:label>Wegde Woreda</rdfs:label>
    </owl:NamedIndividual>
    


    <!-- http://purl.obolibrary.org/obo/GAZ_00123459 -->

    <owl:NamedIndividual rdf:about="http://purl.obolibrary.org/obo/GAZ_00123459">
        <obo:RO_0001025 rdf:resource="http://purl.obolibrary.org/obo/GAZ_00031094"/>
        <obo:IAO_0000115>One of the 105 woredas in the Amhara Region of Ethiopia. Located at the eastern edge of the Ethiopian highlands in the Debub Wollo Zone, Tehuledere is bordered on the south by Dessie Zuria, on the southwest by Kutaber, on the west by Amba Sel, on the north by the Semien Wollo Zone, and on the east by Were Babu. Towns in Tehuledere include Baso Mille, Boru Selassie, Hayq and Sulula.</obo:IAO_0000115>
        <oboInOwl:hasOBONamespace>GAZ</oboInOwl:hasOBONamespace>
        <oboInOwl:id>GAZ:00123459</oboInOwl:id>
        <rdfs:label>Tehuledere Woreda</rdfs:label>
    </owl:NamedIndividual>
    


    <!-- http://purl.obolibrary.org/obo/GAZ_00123460 -->

    <owl:NamedIndividual rdf:about="http://purl.obolibrary.org/obo/GAZ_00123460">
        <obo:RO_0001025 rdf:resource="http://purl.obolibrary.org/obo/GAZ_00031094"/>
        <obo:IAO_0000115>One of the 105 woredas in the Amhara Region of Ethiopia. It is named after the historic district of Sayint. Part of the Debub Wollo Zone, Sayint is bordered on the south by Debre Sina, on the west by the Abay River which separates it from the Misraq Gojjam Zone, on the northwest by the Bashilo River which separates it from the Debub Gondar Zone, on the north by Magdala, on the east by Tenta and on the southeast by Legambo. The major town in Sayint is Sayint Ajebar.</obo:IAO_0000115>
        <oboInOwl:hasOBONamespace>GAZ</oboInOwl:hasOBONamespace>
        <oboInOwl:id>GAZ:00123460</oboInOwl:id>
        <rdfs:label>Sayint Woreda</rdfs:label>
    </owl:NamedIndividual>
    


    <!-- http://purl.obolibrary.org/obo/GAZ_00123461 -->

    <owl:NamedIndividual rdf:about="http://purl.obolibrary.org/obo/GAZ_00123461">
        <obo:RO_0001025 rdf:resource="http://purl.obolibrary.org/obo/GAZ_00031094"/>
        <obo:IAO_0000115>One of the 105 woredas in the Amhara Region of Ethiopia. Part of the Debub Wollo Zone, Kutaber is bordered on the south by Dessie Zuria, on the west by Tenta, on the north by Amba Sel, and on the east by Tehuledere. The major town in Kutaber is Kutaber.</obo:IAO_0000115>
        <oboInOwl:hasOBONamespace>GAZ</oboInOwl:hasOBONamespace>
        <oboInOwl:id>GAZ:00123461</oboInOwl:id>
        <rdfs:label>Kutaber Woreda</rdfs:label>
    </owl:NamedIndividual>
    


    <!-- http://purl.obolibrary.org/obo/GAZ_00123462 -->

    <owl:NamedIndividual rdf:about="http://purl.obolibrary.org/obo/GAZ_00123462">
        <obo:RO_0001025 rdf:resource="http://purl.obolibrary.org/obo/GAZ_00031094"/>
        <obo:IAO_0000115>One of the 105 woredas in the Amhara Region of Ethiopia. Part of the Debub Wollo Zone, Tenta is bordered on the south by Legambo, on the southwest by Sayint, on the west by Magdala, on the north by the Semien Wollo Zone, on the northeast by Amba Sel, on the east by Kutaber and on the southeast by Dessie Zuria. The administrative center of this woreda is Ajebar; other towns in Tenta include Amba Mariam and Tenta.</obo:IAO_0000115>
        <oboInOwl:hasOBONamespace>GAZ</oboInOwl:hasOBONamespace>
        <oboInOwl:id>GAZ:00123462</oboInOwl:id>
        <rdfs:label>Tenta Woreda</rdfs:label>
    </owl:NamedIndividual>
    


    <!-- http://purl.obolibrary.org/obo/GAZ_00123463 -->

    <owl:NamedIndividual rdf:about="http://purl.obolibrary.org/obo/GAZ_00123463">
        <obo:RO_0001025 rdf:resource="http://purl.obolibrary.org/obo/GAZ_00031094"/>
        <obo:IAO_0000115>One of the 105 woredas in the Amhara Region of Ethiopia. Part of the Debub Wollo Zone, Were Babu is bordered on the south by Kalu, on the west by Tehuledere, on the north by the Semien Wollo Zone, on the east by the Afar Region, and on the southeast by the Oromia Zone. Towns in Were Babu include Bistma and Bokeksa.</obo:IAO_0000115>
        <oboInOwl:hasOBONamespace>GAZ</oboInOwl:hasOBONamespace>
        <oboInOwl:id>GAZ:00123463</oboInOwl:id>
        <rdfs:label>Were Babu Woreda</rdfs:label>
    </owl:NamedIndividual>
    


    <!-- http://purl.obolibrary.org/obo/GAZ_00123464 -->

    <owl:NamedIndividual rdf:about="http://purl.obolibrary.org/obo/GAZ_00123464">
        <obo:RO_0001025 rdf:resource="http://purl.obolibrary.org/obo/GAZ_00031094"/>
        <obo:IAO_0000115>One of the 105 woredas in the Amhara Region of Ethiopia. Part of the Debub Wollo Zone, Magdala is bordered on the southwest by Sayint, on the north by the Bashilo River which separates it from the Semien Wollo Zone, and on the east by Tenta. The major town in Magdala is Masha.</obo:IAO_0000115>
        <oboInOwl:hasOBONamespace>GAZ</oboInOwl:hasOBONamespace>
        <oboInOwl:id>GAZ:00123464</oboInOwl:id>
        <rdfs:label>Magdala Woreda</rdfs:label>
    </owl:NamedIndividual>
    


    <!-- http://purl.obolibrary.org/obo/GAZ_00123465 -->

    <owl:NamedIndividual rdf:about="http://purl.obolibrary.org/obo/GAZ_00123465">
        <obo:RO_0001025 rdf:resource="http://purl.obolibrary.org/obo/GAZ_00031094"/>
        <obo:IAO_0000115>One of the 105 woredas of the Amhara Region in Ethiopia, and an amba, or mountain fortress, located in the woreda; the woreda is named for this feature. Located in the Debub Wollo Zone, Ambassel woreda is bordered on the west by Tenta, on the north by the Semien Wollo Zone, on the east by Were Babu, and on the south by Kutaber. Its largest town is Wuchale.</obo:IAO_0000115>
        <oboInOwl:hasOBONamespace>GAZ</oboInOwl:hasOBONamespace>
        <oboInOwl:id>GAZ:00123465</oboInOwl:id>
        <rdfs:label>Amba Sel Woreda</rdfs:label>
    </owl:NamedIndividual>
    


    <!-- http://purl.obolibrary.org/obo/GAZ_00123466 -->

    <owl:NamedIndividual rdf:about="http://purl.obolibrary.org/obo/GAZ_00123466">
        <obo:RO_0001025 rdf:resource="http://purl.obolibrary.org/obo/GAZ_00031094"/>
        <obo:IAO_0000115>One of the 105 woredas in the Amhara Region of Ethiopia. Part of the Debub Wollo Zone, Kelala is bordered on the south by the Semien Shewa Zone, on the southwest by the Walaqa River which separates it from the Oromia Region, on the west by Wegde, on the north by Legambo, on the northeast by Were Ilu, and on the east by Jama. Towns in Kelala include Kelala and Liguama.</obo:IAO_0000115>
        <oboInOwl:hasOBONamespace>GAZ</oboInOwl:hasOBONamespace>
        <oboInOwl:id>GAZ:00123466</oboInOwl:id>
        <rdfs:label>Kelala Woreda</rdfs:label>
    </owl:NamedIndividual>
    


    <!-- http://purl.obolibrary.org/obo/GAZ_00123467 -->

    <owl:NamedIndividual rdf:about="http://purl.obolibrary.org/obo/GAZ_00123467">
        <obo:RO_0001025 rdf:resource="http://purl.obolibrary.org/obo/GAZ_00031094"/>
        <obo:IAO_0000115>One of the 105 woredas in the Amhara Region of Ethiopia. Located at the eastern edge of the Ethiopian highlands in the Debub Wollo Zone, Dessie Zuria is bordered on the south by Were Ilu, on the west by Legambo, on the northwest by Tenta, on the north by Kutaber, on the northeast by Tehuledere, on the east by Kalu, and on the southeast by the Oromia Zone. The cities of Kombolcha and Dessie are independent woredas surrounded by Dessie Zuria; the major town in the woreda is Tita.</obo:IAO_0000115>
        <oboInOwl:hasOBONamespace>GAZ</oboInOwl:hasOBONamespace>
        <oboInOwl:id>GAZ:00123467</oboInOwl:id>
        <rdfs:label>Dessie Zuria Woreda</rdfs:label>
    </owl:NamedIndividual>
    


    <!-- http://purl.obolibrary.org/obo/GAZ_00123468 -->

    <owl:NamedIndividual rdf:about="http://purl.obolibrary.org/obo/GAZ_00123468">
        <obo:RO_0001025 rdf:resource="http://purl.obolibrary.org/obo/GAZ_00031094"/>
        <obo:IAO_0000115>One of the 105 woredas in the Amhara Region of Ethiopia. Part of the Debub Wollo Zone, Jama is bordered on the south and east by the Qechene River which separates it from the Semien Shewa Zone, on the west by Kelala, and on the north by Were Ilu. Towns in Jama include Degolo and Shul Afaf.</obo:IAO_0000115>
        <oboInOwl:hasOBONamespace>GAZ</oboInOwl:hasOBONamespace>
        <oboInOwl:id>GAZ:00123468</oboInOwl:id>
        <rdfs:label>Jama Woreda</rdfs:label>
    </owl:NamedIndividual>
    


    <!-- http://purl.obolibrary.org/obo/GAZ_00123469 -->

    <owl:NamedIndividual rdf:about="http://purl.obolibrary.org/obo/GAZ_00123469">
        <obo:RO_0001025 rdf:resource="http://purl.obolibrary.org/obo/GAZ_00031094"/>
        <obo:IAO_0000115>One of the 105 woredas in the Amhara Region of Ethiopia. Part of the Debub Wollo Zone, Kalu is bordered on the on the west by Dessie Zuria, on the north by Were Babu, and on the south and east by the Oromia Zone. Towns in Kalu include Ancharo, Degaga and Harbu.</obo:IAO_0000115>
        <oboInOwl:hasOBONamespace>GAZ</oboInOwl:hasOBONamespace>
        <oboInOwl:id>GAZ:00123469</oboInOwl:id>
        <rdfs:label>Kalu Woreda</rdfs:label>
    </owl:NamedIndividual>
    


    <!-- http://purl.obolibrary.org/obo/GAZ_00123470 -->

    <owl:NamedIndividual rdf:about="http://purl.obolibrary.org/obo/GAZ_00123470">
        <obo:RO_0001025 rdf:resource="http://purl.obolibrary.org/obo/GAZ_00031094"/>
        <obo:IAO_0000115>One of the 105 woredas in the Amhara Region of Ethiopia. Part of the Debub Wollo Zone, Legambo is bordered on the south by Kelala, on the southwest by Wegde, on the west by Debre Sina, on the northwest by Sayint, on the north by Tenta, on the northeast by Kutaber, on the east by Dessie Zuria, and on the southeast by Were Ilu. Towns in Legambo include Akesta and Embacheber.</obo:IAO_0000115>
        <oboInOwl:hasOBONamespace>GAZ</oboInOwl:hasOBONamespace>
        <oboInOwl:id>GAZ:00123470</oboInOwl:id>
        <rdfs:label>Legambo Woreda</rdfs:label>
    </owl:NamedIndividual>
    


    <!-- http://purl.obolibrary.org/obo/GAZ_00123471 -->

    <owl:NamedIndividual rdf:about="http://purl.obolibrary.org/obo/GAZ_00123471">
        <obo:RO_0001025 rdf:resource="http://purl.obolibrary.org/obo/GAZ_00031094"/>
        <obo:IAO_0000115>A woreda in north-central Ethiopia. Located in the Debub Wollo Zone of the Amhara Region.</obo:IAO_0000115>
        <oboInOwl:hasOBONamespace>GAZ</oboInOwl:hasOBONamespace>
        <oboInOwl:id>GAZ:00123471</oboInOwl:id>
        <rdfs:label>Kombolcha Woreda</rdfs:label>
    </owl:NamedIndividual>
    


    <!-- http://purl.obolibrary.org/obo/GAZ_00123472 -->

    <owl:NamedIndividual rdf:about="http://purl.obolibrary.org/obo/GAZ_00123472">
        <obo:RO_0001025 rdf:resource="http://purl.obolibrary.org/obo/GAZ_00031094"/>
        <obo:IAO_0000115>A woreda in north-central Ethiopia.</obo:IAO_0000115>
        <oboInOwl:hasOBONamespace>GAZ</oboInOwl:hasOBONamespace>
        <oboInOwl:id>GAZ:00123472</oboInOwl:id>
        <rdfs:label>Dessie Woreda</rdfs:label>
    </owl:NamedIndividual>
    


    <!-- http://purl.obolibrary.org/obo/GAZ_00123473 -->

    <owl:NamedIndividual rdf:about="http://purl.obolibrary.org/obo/GAZ_00123473">
        <obo:RO_0001025 rdf:resource="http://purl.obolibrary.org/obo/GAZ_00123459"/>
        <obo:IAO_0000115>A lake S of Lake Hayq.</obo:IAO_0000115>
        <oboInOwl:hasOBONamespace>GAZ</oboInOwl:hasOBONamespace>
        <oboInOwl:id>GAZ:00123473</oboInOwl:id>
        <rdfs:label>Lake Ardibbo</rdfs:label>
    </owl:NamedIndividual>
    


    <!-- http://purl.obolibrary.org/obo/GAZ_00123474 -->

    <owl:NamedIndividual rdf:about="http://purl.obolibrary.org/obo/GAZ_00123474">
        <obo:RO_0001025 rdf:resource="http://purl.obolibrary.org/obo/GAZ_00031100"/>
        <obo:IAO_0000115>One of the 105 woredas in the Amhara Region of Ethiopia. Part of the Mirab Gojjam Zone, Jabi Tehnan is bordered on the southeast by Dembecha, on the west by Bure Wemberma, on the northwest by Sekela, on the north by Kuarit, and on the east by Bibugn. Towns in Jabi Tehnan include Finote Selam, Jiga, Maksegnit and Mankusa.</obo:IAO_0000115>
        <oboInOwl:hasOBONamespace>GAZ</oboInOwl:hasOBONamespace>
        <oboInOwl:id>GAZ:00123474</oboInOwl:id>
        <rdfs:label>Jabi Tehnant Woreda</rdfs:label>
    </owl:NamedIndividual>
    


    <!-- http://purl.obolibrary.org/obo/GAZ_00123475 -->

    <owl:NamedIndividual rdf:about="http://purl.obolibrary.org/obo/GAZ_00123475">
        <obo:RO_0001025 rdf:resource="http://purl.obolibrary.org/obo/GAZ_00031100"/>
        <obo:IAO_0000115>One of the 105 woredas in the Amhara Region of Ethiopia. Part of the Mirab Gojjam Zone, Achefer is bordered on the south by the Agew Awi Zone, on the west by the Semien Gondar Zone, on the north by Lake Tana, on the northeast by Bahir Dar Zuria, and on the southeast by Merawi; the Lesser Abay River defines the woreda&apos;s eastern boundary. The woreda includes Dek Island. Towns in Achefer include Durbete, Kunzela and Yesmala.</obo:IAO_0000115>
        <oboInOwl:hasOBONamespace>GAZ</oboInOwl:hasOBONamespace>
        <oboInOwl:id>GAZ:00123475</oboInOwl:id>
        <rdfs:label>Achefert Woreda</rdfs:label>
    </owl:NamedIndividual>
    


    <!-- http://purl.obolibrary.org/obo/GAZ_00123476 -->

    <owl:NamedIndividual rdf:about="http://purl.obolibrary.org/obo/GAZ_00123476">
        <obo:RO_0001025 rdf:resource="http://purl.obolibrary.org/obo/GAZ_00031100"/>
        <obo:IAO_0000115>One of the 105 woredas in the Amhara Region of Ethiopia. Part of the Mirab Gojjam Zone, Sekela is bordered on the southwest by Bure Wemberma, on the west by the Agew Awi Zone, on the north by Merawi, on the northeast by Adet, on the east by Kuarit, and on the southeast by Jabi Tehnan. The major town in Sekela is Gish Abay.</obo:IAO_0000115>
        <oboInOwl:hasOBONamespace>GAZ</oboInOwl:hasOBONamespace>
        <oboInOwl:id>GAZ:00123476</oboInOwl:id>
        <rdfs:label>Sekelat Woreda</rdfs:label>
    </owl:NamedIndividual>
    


    <!-- http://purl.obolibrary.org/obo/GAZ_00123477 -->

    <owl:NamedIndividual rdf:about="http://purl.obolibrary.org/obo/GAZ_00123477">
        <obo:RO_0001025 rdf:resource="http://purl.obolibrary.org/obo/GAZ_00031100"/>
        <obo:IAO_0000115>One of the 105 woredas in the Amhara Region of Ethiopia. Part of the Mirab Gojjam Zone, Dembecha is bordered on the west by Bure Wemberma, on the northwest by Jabi Tehnan, on the north by Bibugn, and on the east and south by the Misraq Gojjam Zone. Towns in Dembecha include Addis Alem, Dembecha and Yechereka.</obo:IAO_0000115>
        <oboInOwl:hasOBONamespace>GAZ</oboInOwl:hasOBONamespace>
        <oboInOwl:id>GAZ:00123477</oboInOwl:id>
        <rdfs:label>Dembechat Woreda</rdfs:label>
    </owl:NamedIndividual>
    


    <!-- http://purl.obolibrary.org/obo/GAZ_00123478 -->

    <owl:NamedIndividual rdf:about="http://purl.obolibrary.org/obo/GAZ_00123478">
        <obo:RO_0001025 rdf:resource="http://purl.obolibrary.org/obo/GAZ_00031100"/>
        <obo:IAO_0000115>One of the 105 woredas in the Amhara Region of Ethiopia. Part of the Mirab Gojjam Zone, Merawi is bordered on the south by Sekela, on the west by the Agew Awi Zone, on the northwest by the Lesser Abay River which spearates it from Achefer, on the northeast by Bahir Dar Zuria, and on the east by Adet. Towns in Merawi include Merawi and Wetet Abay.</obo:IAO_0000115>
        <oboInOwl:hasOBONamespace>GAZ</oboInOwl:hasOBONamespace>
        <oboInOwl:id>GAZ:00123478</oboInOwl:id>
        <rdfs:label>Merawit Woreda</rdfs:label>
    </owl:NamedIndividual>
    


    <!-- http://purl.obolibrary.org/obo/GAZ_00123479 -->

    <owl:NamedIndividual rdf:about="http://purl.obolibrary.org/obo/GAZ_00123479">
        <obo:RO_0001025 rdf:resource="http://purl.obolibrary.org/obo/GAZ_00031100"/>
        <obo:IAO_0000115>One of the 105 woredas in the Amhara Region of Ethiopia. Part of the Mirab Gojjam Zone, Dega Damot is bordered on the south for a short length by Dembecha, on the southwest by Jabi Tehnan, on the northwest by Kuarit, and on the east and south by the Misraq Gojjam Zone. The major town in Dega Damot is Feres Bet.</obo:IAO_0000115>
        <oboInOwl:hasOBONamespace>GAZ</oboInOwl:hasOBONamespace>
        <oboInOwl:id>GAZ:00123479</oboInOwl:id>
        <rdfs:label>Dega Damott Woreda</rdfs:label>
    </owl:NamedIndividual>
    


    <!-- http://purl.obolibrary.org/obo/GAZ_00123480 -->

    <owl:NamedIndividual rdf:about="http://purl.obolibrary.org/obo/GAZ_00123480">
        <obo:RO_0001025 rdf:resource="http://purl.obolibrary.org/obo/GAZ_00031100"/>
        <obo:IAO_0000115>One of the 105 woredas in the Amhara Region of Ethiopia. Part of the Mirab Gojjam Zone, this woreda is bordered on the south by Adet, on the southwest by Merawi, on the northwest by the Lesser Abay River which separates it from Achefer, on the north by Lake Tana, on the northeast by the city and special zone of Bahir Dar, and on the east by the Abay River which separates it from the Debub Gondar Zone. Towns in Bahir Dar Zuria include Meshenti, Tis Abay and Zege.</obo:IAO_0000115>
        <oboInOwl:hasOBONamespace>GAZ</oboInOwl:hasOBONamespace>
        <oboInOwl:id>GAZ:00123480</oboInOwl:id>
        <rdfs:label>Bahir Dar Zuriat Woreda</rdfs:label>
    </owl:NamedIndividual>
    


    <!-- http://purl.obolibrary.org/obo/GAZ_00123481 -->

    <owl:NamedIndividual rdf:about="http://purl.obolibrary.org/obo/GAZ_00123481">
        <obo:RO_0001025 rdf:resource="http://purl.obolibrary.org/obo/GAZ_00031100"/>
        <obo:IAO_0000115>One of the 105 woredas in the Amhara Region of Ethiopia. Part of the Mirab Gojjam Zone, Bure Wemberma is bordered on the south by the Abay River which separates it from the Oromia Region, on the west by the Agew Awi Zone, on the north by Sekela, on the northeast by Jabi Tehnan, on the east by Bibugn, and on the southeast by the Misraq Gojjam Zone. Towns in Bure Wemberma include Shendi.</obo:IAO_0000115>
        <oboInOwl:hasOBONamespace>GAZ</oboInOwl:hasOBONamespace>
        <oboInOwl:id>GAZ:00123481</oboInOwl:id>
        <rdfs:label>Bure Wembermat Woreda</rdfs:label>
    </owl:NamedIndividual>
    


    <!-- http://purl.obolibrary.org/obo/GAZ_00123482 -->

    <owl:NamedIndividual rdf:about="http://purl.obolibrary.org/obo/GAZ_00123482">
        <obo:RO_0001025 rdf:resource="http://purl.obolibrary.org/obo/GAZ_00031100"/>
        <obo:IAO_0000115>One of the 105 woredas in the Amhara Region of Ethiopia. Part of the Mirab Gojjam Zone, Kuarit is bordered on the southwest by Jabi Tehnan, on the west by Sekela, on the north by Adet, on the east by the Misraq Gojjam Zone, and on the southeast by Dega Damot. The major town in Kuarit is Gebeze Mariam.</obo:IAO_0000115>
        <oboInOwl:hasOBONamespace>GAZ</oboInOwl:hasOBONamespace>
        <oboInOwl:id>GAZ:00123482</oboInOwl:id>
        <rdfs:label>Kuaritt Woreda</rdfs:label>
    </owl:NamedIndividual>
    


    <!-- http://purl.obolibrary.org/obo/GAZ_00123483 -->

    <owl:NamedIndividual rdf:about="http://purl.obolibrary.org/obo/GAZ_00123483">
        <obo:RO_0001025 rdf:resource="http://purl.obolibrary.org/obo/GAZ_00031100"/>
        <obo:IAO_0000115>One of the 105 woredas in the Amhara Region of Ethiopia. Part of the Mirab Gojjam Zone, Adet is bordered on the south by Kuarit, on the southwest by Sekela, on the west by Merawi, on the north by Bahir Dar Zuria, on the east by the Abay River which separates it from the Debub Gondar Zone, and on the southeast by the Misraq Gojjam Zone. The major town in Adet is Adet.</obo:IAO_0000115>
        <oboInOwl:hasOBONamespace>GAZ</oboInOwl:hasOBONamespace>
        <oboInOwl:id>GAZ:00123483</oboInOwl:id>
        <rdfs:label>Adet Woreda</rdfs:label>
    </owl:NamedIndividual>
    


    <!-- http://purl.obolibrary.org/obo/GAZ_00123484 -->

    <owl:NamedIndividual rdf:about="http://purl.obolibrary.org/obo/GAZ_00123484">
        <obo:RO_0001025 rdf:resource="http://purl.obolibrary.org/obo/GAZ_00031103"/>
        <obo:IAO_0000115>A woreda in east-central Ethiopia. Located in the Misraq Gojjam Zone of the Amhara Region.</obo:IAO_0000115>
        <oboInOwl:hasOBONamespace>GAZ</oboInOwl:hasOBONamespace>
        <oboInOwl:id>GAZ:00123484</oboInOwl:id>
        <rdfs:label>Debre Marqos Woreba</rdfs:label>
    </owl:NamedIndividual>
    


    <!-- http://purl.obolibrary.org/obo/GAZ_00123485 -->

    <owl:NamedIndividual rdf:about="http://purl.obolibrary.org/obo/GAZ_00123485">
        <obo:RO_0001025 rdf:resource="http://purl.obolibrary.org/obo/GAZ_00031103"/>
        <obo:IAO_0000115>One of the 105 woredas in the Amhara Region of Ethiopia. Part of the Misraq Gojjam Zone, Bibugn is bordered on the south by Machakel, on the west by the Mirab Gojjam Zone, and on the east by Hulet Ej Enese. Towns in Bibugn include Digua Tsion and Weyin.</obo:IAO_0000115>
        <oboInOwl:hasOBONamespace>GAZ</oboInOwl:hasOBONamespace>
        <oboInOwl:id>GAZ:00123485</oboInOwl:id>
        <rdfs:label>Bibugn Woreba</rdfs:label>
    </owl:NamedIndividual>
    


    <!-- http://purl.obolibrary.org/obo/GAZ_00123486 -->

    <owl:NamedIndividual rdf:about="http://purl.obolibrary.org/obo/GAZ_00123486">
        <obo:RO_0001025 rdf:resource="http://purl.obolibrary.org/obo/GAZ_00031103"/>
        <obo:IAO_0000115>One of the 105 woredas in the Amhara Region of Ethiopia. Part of the Misraq Gojjam Zone, Shebel Berenta is bordered on the southwest by Dejen, on the northwest by Enemay, on the north by Enarj Enawga, and on the east by the Abay River which separates it from the Oromia Region. The major town in Shebel Berenta is Yed Wuha.</obo:IAO_0000115>
        <oboInOwl:hasOBONamespace>GAZ</oboInOwl:hasOBONamespace>
        <oboInOwl:id>GAZ:00123486</oboInOwl:id>
        <rdfs:label>Shebel Berenta Woreba</rdfs:label>
    </owl:NamedIndividual>
    


    <!-- http://purl.obolibrary.org/obo/GAZ_00123487 -->

    <owl:NamedIndividual rdf:about="http://purl.obolibrary.org/obo/GAZ_00123487">
        <obo:RO_0001025 rdf:resource="http://purl.obolibrary.org/obo/GAZ_00031103"/>
        <obo:IAO_0000115>One of the 105 woredas in the Amhara Region of Ethiopia. Part of the Misraq Gojjam Zone, Debay Telatgen is bordered on the extreme south by Dejen, on the further southwest by Awabel, on the closer southwest by Guzamn, on the west by Machakel, on the northwest by Bibugn, on the north by Hulet Ej Enese, on the northeast by Enarj Enawga, and on the east by Enemay. The major town in Debay Telatgen is Kuyi.</obo:IAO_0000115>
        <oboInOwl:hasOBONamespace>GAZ</oboInOwl:hasOBONamespace>
        <oboInOwl:id>GAZ:00123487</oboInOwl:id>
        <rdfs:label>Debay Telatgen Woreba</rdfs:label>
    </owl:NamedIndividual>
    


    <!-- http://purl.obolibrary.org/obo/GAZ_00123488 -->

    <owl:NamedIndividual rdf:about="http://purl.obolibrary.org/obo/GAZ_00123488">
        <obo:RO_0001025 rdf:resource="http://purl.obolibrary.org/obo/GAZ_00031103"/>
        <obo:IAO_0000115>One of the 105 woredas in the Amhara Region of Ethiopia. Part of the Misraq Gojjam Zone, Guzamn is bordered on the south by Baso Liben, on the southwest by the Abay River which separates it from the Oromia Region, on the west by Machakel, on the northwest by Debay Telatgen, and on the east by Awabel; the town and woreda of Debre Marqos is an enclave inside Guzamn. Towns in Guzamn include Chemoga, Rob Gebeya and Yebokile.</obo:IAO_0000115>
        <oboInOwl:hasOBONamespace>GAZ</oboInOwl:hasOBONamespace>
        <oboInOwl:id>GAZ:00123488</oboInOwl:id>
        <rdfs:label>Guzamn Woreba</rdfs:label>
    </owl:NamedIndividual>
    


    <!-- http://purl.obolibrary.org/obo/GAZ_00123489 -->

    <owl:NamedIndividual rdf:about="http://purl.obolibrary.org/obo/GAZ_00123489">
        <obo:RO_0001025 rdf:resource="http://purl.obolibrary.org/obo/GAZ_00031103"/>
        <obo:IAO_0000115>One of the 105 woredas in the Amhara Region of Ethiopia. Part of the Misraq Gojjam Zone, Dejen is bordered on the south by the Abay River which separates it from the Oromia Region, on the west by Awabel, on the northwest by Enarj Enawga, on the north by Enemay, and on the east by Shebel Berenta. The major town in Dejen is Dejen.</obo:IAO_0000115>
        <oboInOwl:hasOBONamespace>GAZ</oboInOwl:hasOBONamespace>
        <oboInOwl:id>GAZ:00123489</oboInOwl:id>
        <rdfs:label>Dejen Woreba</rdfs:label>
    </owl:NamedIndividual>
    


    <!-- http://purl.obolibrary.org/obo/GAZ_00123490 -->

    <owl:NamedIndividual rdf:about="http://purl.obolibrary.org/obo/GAZ_00123490">
        <obo:RO_0001025 rdf:resource="http://purl.obolibrary.org/obo/GAZ_00031103"/>
        <obo:IAO_0000115>One of the 105 woredas in the Amhara Region of Ethiopia. Part of the Misraq Gojjam Zone, Enemay is bordered on the south by Dejen, on the west by Debay Telatgen, on the north by Enarj Enawga, and on the east by Shebel Berenta. Towns in Enemay include Bichena and Yetmen.</obo:IAO_0000115>
        <oboInOwl:hasOBONamespace>GAZ</oboInOwl:hasOBONamespace>
        <oboInOwl:id>GAZ:00123490</oboInOwl:id>
        <rdfs:label>Enemay Woreba</rdfs:label>
    </owl:NamedIndividual>
    


    <!-- http://purl.obolibrary.org/obo/GAZ_00123491 -->

    <owl:NamedIndividual rdf:about="http://purl.obolibrary.org/obo/GAZ_00123491">
        <obo:RO_0001025 rdf:resource="http://purl.obolibrary.org/obo/GAZ_00031103"/>
        <obo:IAO_0000115>One of the 105 woredas in the Amhara Region of Ethiopia. Part of the Misraq Gojjam Zone, Enbise Sar Midir is bordered on the south by Enarj Enawga, on the west by Goncha Siso Enese, and on the north and east by Abay River which separates it from the Debub Wollo Zone. The woreda capital is Merto Lemariam; other towns in Enbise Sar Midir include Dibo.</obo:IAO_0000115>
        <oboInOwl:hasOBONamespace>GAZ</oboInOwl:hasOBONamespace>
        <oboInOwl:id>GAZ:00123491</oboInOwl:id>
        <rdfs:label>Enbise Sar Midir Woreba</rdfs:label>
    </owl:NamedIndividual>
    


    <!-- http://purl.obolibrary.org/obo/GAZ_00123492 -->

    <owl:NamedIndividual rdf:about="http://purl.obolibrary.org/obo/GAZ_00123492">
        <obo:RO_0001025 rdf:resource="http://purl.obolibrary.org/obo/GAZ_00031103"/>
        <obo:IAO_0000115>One of the 105 woredas in the Amhara Region of Ethiopia. A triangular-shaped district in the Misraq Gojjam Zone, Baso Liben is bordered on the south by the Abay River which separates it from the Oromia Region, on the northwest by Guzamn, and on the northeast by Awabel. The major town in Baso Liben is Yejube.</obo:IAO_0000115>
        <oboInOwl:hasOBONamespace>GAZ</oboInOwl:hasOBONamespace>
        <oboInOwl:id>GAZ:00123492</oboInOwl:id>
        <rdfs:label>Baso Liben Woreba</rdfs:label>
    </owl:NamedIndividual>
    


    <!-- http://purl.obolibrary.org/obo/GAZ_00123493 -->

    <owl:NamedIndividual rdf:about="http://purl.obolibrary.org/obo/GAZ_00123493">
        <obo:RO_0001025 rdf:resource="http://purl.obolibrary.org/obo/GAZ_00031103"/>
        <obo:IAO_0000115>One of the 105 woredas in the Amhara Region of Ethiopia. Part of the Misraq Gojjam Zone, Goncha Siso Enese is bordered on the south by Enarj Enawga, on the west by Hulet Ej Enese, on the north by the Abay River which separates it from the Debub Gondar Zone, and on the east by Enbise Sar Midir. The major town in Goncha Siso Enese is Gindo Weyin.</obo:IAO_0000115>
        <oboInOwl:hasOBONamespace>GAZ</oboInOwl:hasOBONamespace>
        <oboInOwl:id>GAZ:00123493</oboInOwl:id>
        <rdfs:label>Goncha Siso Enese Woreba</rdfs:label>
    </owl:NamedIndividual>
    


    <!-- http://purl.obolibrary.org/obo/GAZ_00123494 -->

    <owl:NamedIndividual rdf:about="http://purl.obolibrary.org/obo/GAZ_00123494">
        <obo:RO_0001025 rdf:resource="http://purl.obolibrary.org/obo/GAZ_00031103"/>
        <obo:IAO_0000115>One of the 105 woredas in the Amhara Region of Ethiopia. Part of the Misraq Gojjam Zone, Hulet Ej Enese is bordered on the south by Debay Telatgen, on the southwest by Bibugn, on the northwest by the Mirab Gojjam Zone, on the north by the Abay River which separates it from the Debub Gondar Zone, on the east by Goncha Siso Enese, and on the southeast by Enarj Enawga. Towns in this woreda include Keraniyo, Mota and Sede.</obo:IAO_0000115>
        <oboInOwl:hasOBONamespace>GAZ</oboInOwl:hasOBONamespace>
        <oboInOwl:id>GAZ:00123494</oboInOwl:id>
        <rdfs:label>Hulet Ej Enese Woreba</rdfs:label>
    </owl:NamedIndividual>
    


    <!-- http://purl.obolibrary.org/obo/GAZ_00123495 -->

    <owl:NamedIndividual rdf:about="http://purl.obolibrary.org/obo/GAZ_00123495">
        <obo:RO_0001025 rdf:resource="http://purl.obolibrary.org/obo/GAZ_00031103"/>
        <obo:IAO_0000115>One of the 105 woredas in the Amhara Region of Ethiopia. Part of the Misraq Gojjam Zone, Enarj Enawga is bordered on the south by Enemay, on the southwest by Debay Telatgen, on the west by Hulet Ej Enese, on the north by Goncha Siso Enese, on the northeast by Enbise Sar Midir, on the east by the Abbay River which separates it from the Debub Wollo Zone, and on the southeast by Shebel Berenta. Towns in Enarj Enawga include Debre Werq and Felege Berhan.</obo:IAO_0000115>
        <oboInOwl:hasOBONamespace>GAZ</oboInOwl:hasOBONamespace>
        <oboInOwl:id>GAZ:00123495</oboInOwl:id>
        <rdfs:label>Enarj Enawga Woreba</rdfs:label>
    </owl:NamedIndividual>
    


    <!-- http://purl.obolibrary.org/obo/GAZ_00123496 -->

    <owl:NamedIndividual rdf:about="http://purl.obolibrary.org/obo/GAZ_00123496">
        <obo:RO_0001025 rdf:resource="http://purl.obolibrary.org/obo/GAZ_00031103"/>
        <obo:IAO_0000115>One of the 105 woredas in the Amhara Region of Ethiopia. Part of the Misraq Gojjam Zone, Machakel is bordered on the south by the Abay River which separates it from the Oromia Region, on the west by the Mirab Gojjam Zone, on the north by Bibugn, and on the east by Guzamn. Towns in Machakel include Amanuel and Elias.</obo:IAO_0000115>
        <oboInOwl:hasOBONamespace>GAZ</oboInOwl:hasOBONamespace>
        <oboInOwl:id>GAZ:00123496</oboInOwl:id>
        <rdfs:label>Machakel Woreba</rdfs:label>
    </owl:NamedIndividual>
    


    <!-- http://purl.obolibrary.org/obo/GAZ_00123497 -->

    <owl:NamedIndividual rdf:about="http://purl.obolibrary.org/obo/GAZ_00123497">
        <obo:RO_0001025 rdf:resource="http://purl.obolibrary.org/obo/GAZ_00031103"/>
        <obo:IAO_0000115>One of the 105 woredas in the Amhara Region of Ethiopia. Part of the Misraq Gojjam Zone, Awabel is bordered on the south by the Abay River which separates it from the Oromia Region, on the southwest by Baso Liben, on the northwest by Guzamn, on the northeast by Enemay, and on the southeast by Dejen. Towns in Awabel include Amber, Liga, Lumame and Wejel.</obo:IAO_0000115>
        <oboInOwl:hasOBONamespace>GAZ</oboInOwl:hasOBONamespace>
        <oboInOwl:id>GAZ:00123497</oboInOwl:id>
        <rdfs:label>Awabel Woreba Woreba</rdfs:label>
    </owl:NamedIndividual>
    


    <!-- http://purl.obolibrary.org/obo/GAZ_00123498 -->

    <owl:NamedIndividual rdf:about="http://purl.obolibrary.org/obo/GAZ_00123498">
        <obo:RO_0001025 rdf:resource="http://purl.obolibrary.org/obo/GAZ_00031095"/>
        <obo:IAO_0000115>One of the 105 woredas in the Amhara Region of Ethiopia. Part of the Oromia Zone, Artuma Fursina Jile is bordered on the west by the Semien Shewa Zone, on the north by Chefe Golana Dewerahmedo, and on the east by the Afar Region. Towns in Artuma Fursina Jile include Adebela, Chefa Robit, Kichicho and Senbete.</obo:IAO_0000115>
        <oboInOwl:hasOBONamespace>GAZ</oboInOwl:hasOBONamespace>
        <oboInOwl:id>GAZ:00123498</oboInOwl:id>
        <rdfs:label>Artuma Fursina Jile Woreda</rdfs:label>
    </owl:NamedIndividual>
    


    <!-- http://purl.obolibrary.org/obo/GAZ_00123499 -->

    <owl:NamedIndividual rdf:about="http://purl.obolibrary.org/obo/GAZ_00123499">
        <obo:RO_0001025 rdf:resource="http://purl.obolibrary.org/obo/GAZ_00031095"/>
        <obo:IAO_0000115>One of the 105 woredas in the Amhara Region of Ethiopia. Part of the Oromia Zone, Bati is bordered on the south by Chefe Golana Dewerahmedo, on the west and north by the Debub Wollo Zone, and on the east by the Afar Region. Towns in Bati include Bati, Gerba and Degan.</obo:IAO_0000115>
        <oboInOwl:hasOBONamespace>GAZ</oboInOwl:hasOBONamespace>
        <oboInOwl:id>GAZ:00123499</oboInOwl:id>
        <rdfs:label>Bati Woreda</rdfs:label>
    </owl:NamedIndividual>
    


    <!-- http://purl.obolibrary.org/obo/GAZ_00123500 -->

    <owl:NamedIndividual rdf:about="http://purl.obolibrary.org/obo/GAZ_00123500">
        <obo:RO_0001025 rdf:resource="http://purl.obolibrary.org/obo/GAZ_00031095"/>
        <obo:IAO_0000115>One of the 105 woredas in the Amhara Region of Ethiopia. Part of the Oromia Zone, Chefe Golana Dewerahmedo is bordered on the south by Artuma Fursina Jile, on the southwest by the Semien Shewa Zone, on the west by the Debub Wollo Zone, on the north by Bati, and on the east by the Afar Region. Towns in Chefe Golana Dewerahmedo include Bora and Kemise.</obo:IAO_0000115>
        <oboInOwl:hasOBONamespace>GAZ</oboInOwl:hasOBONamespace>
        <oboInOwl:id>GAZ:00123500</oboInOwl:id>
        <rdfs:label>Chefe Golana Dewerahmedo Woreda</rdfs:label>
    </owl:NamedIndividual>
    


    <!-- http://purl.obolibrary.org/obo/GAZ_00123501 -->

    <owl:NamedIndividual rdf:about="http://purl.obolibrary.org/obo/GAZ_00123501">
        <obo:RO_0001025 rdf:resource="http://purl.obolibrary.org/obo/GAZ_00031097"/>
        <obo:IAO_0000115>One of the 105 woredas in the Amhara Region of Ethiopia. Part of the Wag Hemra Zone, Dehana is bordered on the south by the Semien (North) Wollo Zone, on the southwest by the Debub (South) Gondar Zone, ion the northwest by the Semien (North) Gondar Zone, on the north by Zikuala, and on the east by Soqota. The major town in Dehana is Made Werq.</obo:IAO_0000115>
        <oboInOwl:hasOBONamespace>GAZ</oboInOwl:hasOBONamespace>
        <oboInOwl:id>GAZ:00123501</oboInOwl:id>
        <rdfs:label>Dehana Woreda</rdfs:label>
    </owl:NamedIndividual>
    


    <!-- http://purl.obolibrary.org/obo/GAZ_00123502 -->

    <owl:NamedIndividual rdf:about="http://purl.obolibrary.org/obo/GAZ_00123502">
        <obo:RO_0001025 rdf:resource="http://purl.obolibrary.org/obo/GAZ_00031097"/>
        <obo:IAO_0000115>One of the 105 woredas in the Amhara Region of Ethiopia. Located on the eastern escarpment of the Ethiopian highlands in the Wag Hemra Zone, Soqota is bordered on the south by the Semien Wollo Zone, on the southwest by Dehana, on the northwest by the Tekeze River which separates it from Zikuala, and on the north and east by the Tigray Region. Towns in Soqota include Nirak and Soqota.</obo:IAO_0000115>
        <oboInOwl:hasOBONamespace>GAZ</oboInOwl:hasOBONamespace>
        <oboInOwl:id>GAZ:00123502</oboInOwl:id>
        <rdfs:label>Soqota Woreda</rdfs:label>
    </owl:NamedIndividual>
    


    <!-- http://purl.obolibrary.org/obo/GAZ_00123503 -->

    <owl:NamedIndividual rdf:about="http://purl.obolibrary.org/obo/GAZ_00123503">
        <obo:RO_0001025 rdf:resource="http://purl.obolibrary.org/obo/GAZ_00031097"/>
        <obo:IAO_0000115>One of the 105 woredas in the Amhara Region of Ethiopia. Part of the Wag Hemra Zone, Zikuala is bordered on the south by Dehana, on the west and north by the Debub Gondar Zone, and on the east by the Tekeze River which separates it from Soqota. Other rivers include the Balagas.</obo:IAO_0000115>
        <oboInOwl:hasOBONamespace>GAZ</oboInOwl:hasOBONamespace>
        <oboInOwl:id>GAZ:00123503</oboInOwl:id>
        <rdfs:label>Zikuala Woreda</rdfs:label>
    </owl:NamedIndividual>
    


    <!-- http://purl.obolibrary.org/obo/GAZ_00123504 -->

    <owl:NamedIndividual rdf:about="http://purl.obolibrary.org/obo/GAZ_00123504">
        <obo:RO_0001025 rdf:resource="http://purl.obolibrary.org/obo/GAZ_00031093"/>
        <obo:IAO_0000115>One of the 105 woredas in the Amhara Region of Ethiopia. Part of the Semien Shewa Zone, Berehet is bordered on the south by the Germama River which separates it from Menjarna Shenkora, on the west by Hagere Mariamna Kesem, on the northeast by Angolalla Terana Asagirt, on the north by Ankober, and on the east by the Afar Region. The major town in Berehet is Metiteh Bila.</obo:IAO_0000115>
        <oboInOwl:hasOBONamespace>GAZ</oboInOwl:hasOBONamespace>
        <oboInOwl:id>GAZ:00123504</oboInOwl:id>
        <rdfs:label>Berehet Woreda</rdfs:label>
    </owl:NamedIndividual>
    


    <!-- http://purl.obolibrary.org/obo/GAZ_00123505 -->

    <owl:NamedIndividual rdf:about="http://purl.obolibrary.org/obo/GAZ_00123505">
        <obo:RO_0001025 rdf:resource="http://purl.obolibrary.org/obo/GAZ_00031093"/>
        <obo:IAO_0000115>One of the 105 woredas in the Amhara Region of Ethiopia. Located at the eastern edge of the Ethiopian highlands in the Semien Shewa Zone, Ankober is bordered on the south by Berehet, on the southwest by Angolalla Terana Asagirt, on the northwest by Debre Berhan Zuria, on the north by Kewet, and on the east by the Afar Region. Towns in Ankober include Aliyu Amba, Ankober, Gorgo and Haramba.</obo:IAO_0000115>
        <oboInOwl:hasOBONamespace>GAZ</oboInOwl:hasOBONamespace>
        <oboInOwl:id>GAZ:00123505</oboInOwl:id>
        <rdfs:label>Ankober Woreda</rdfs:label>
    </owl:NamedIndividual>
    


    <!-- http://purl.obolibrary.org/obo/GAZ_00123506 -->

    <owl:NamedIndividual rdf:about="http://purl.obolibrary.org/obo/GAZ_00123506">
        <obo:RO_0001025 rdf:resource="http://purl.obolibrary.org/obo/GAZ_00031093"/>
        <obo:IAO_0000115>One of the 105 woredas in the Amhara Region of Ethiopia. Part of the Semien Shewa Zone, Weremo Wajetuna Midarema is bordered on the south by the Qechene River which separates it from Lay Betna Tach Bet, on the west by the Oromia Region, and on the north and east by the Debub Wollo Zone; the northern boundary is defined by the Walaqa River. The administrative center of this woreda is Meragna; other towns include Rema.</obo:IAO_0000115>
        <oboInOwl:hasOBONamespace>GAZ</oboInOwl:hasOBONamespace>
        <oboInOwl:id>GAZ:00123506</oboInOwl:id>
        <rdfs:label>Weremo Wajetuna Midarema Woreda</rdfs:label>
    </owl:NamedIndividual>
    


    <!-- http://purl.obolibrary.org/obo/GAZ_00123507 -->

    <owl:NamedIndividual rdf:about="http://purl.obolibrary.org/obo/GAZ_00123507">
        <obo:RO_0001025 rdf:resource="http://purl.obolibrary.org/obo/GAZ_00031093"/>
        <obo:IAO_0000115>One of the 105 woredas in the Amhara Region of Ethiopia. Part of the Semien Shewa Zone, Hagere Mariamna Kesem is bordered on the south by the Germama River which separates it from Menjarna Shenkora, on the west and north by the Oromia Region, on the northeast by Angolalla Terana Asagirt, and on the east by Berehet. The administrative center of this woreda is Shola Gebeya; other towns include Kese Koremash.</obo:IAO_0000115>
        <oboInOwl:hasOBONamespace>GAZ</oboInOwl:hasOBONamespace>
        <oboInOwl:id>GAZ:00123507</oboInOwl:id>
        <rdfs:label>Hagere Mariamna Kesem Woreda</rdfs:label>
    </owl:NamedIndividual>
    


    <!-- http://purl.obolibrary.org/obo/GAZ_00123508 -->

    <owl:NamedIndividual rdf:about="http://purl.obolibrary.org/obo/GAZ_00123508">
        <obo:RO_0001025 rdf:resource="http://purl.obolibrary.org/obo/GAZ_00031099"/>
        <obo:IAO_0000115>One of the 105 woredas in the Amhara Region of Ethiopia. Part of the Semien Gondar Zone, Gondar Zuria is bordered on the south by the Debub Gondar Zone, on the southwest by Lake Tana, on the west by Dembiya, on the north by Lay Armachiho, on the northeast by Wegera, and on the southeast by Belessa. Towns and cities in Gondar Zuria include Degoma, Emfraz, Maksenit and Teda. The city and woreda of Gondar is surrounded by Gondar Zuria in the northern part of this woreda.</obo:IAO_0000115>
        <oboInOwl:hasOBONamespace>GAZ</oboInOwl:hasOBONamespace>
        <oboInOwl:id>GAZ:00123508</oboInOwl:id>
        <rdfs:label>Gondar Zuria Woreda</rdfs:label>
    </owl:NamedIndividual>
    


    <!-- http://purl.obolibrary.org/obo/GAZ_00123509 -->

    <owl:NamedIndividual rdf:about="http://purl.obolibrary.org/obo/GAZ_00123509">
        <obo:RO_0001025 rdf:resource="http://purl.obolibrary.org/obo/GAZ_00031093"/>
        <obo:IAO_0000115>One of the 105 woredas in the Amhara Region of Ethiopia. Located at the eastern edge of the Ethiopian highlands in the Semien Shewa Zone, Mafud Mezezo Mojana is bordered on the south by Debre Berhan Zuria, on the west by the Oromia Region, on the northwest by Gera Midira Keya Gebriel, on the north by Mam Midrina Lalo Midir, on the northeast by Kewet, and on the southeast by the Afar Region. The administrative center of this woreda is Sela Dingay; other towns in this woreda include Debre Sina and Mezezo.</obo:IAO_0000115>
        <oboInOwl:hasOBONamespace>GAZ</oboInOwl:hasOBONamespace>
        <oboInOwl:id>GAZ:00123509</oboInOwl:id>
        <rdfs:label>Mafud Mezezo Mojana Woreda</rdfs:label>
    </owl:NamedIndividual>
    


    <!-- http://purl.obolibrary.org/obo/GAZ_00123510 -->

    <owl:NamedIndividual rdf:about="http://purl.obolibrary.org/obo/GAZ_00123510">
        <obo:RO_0001025 rdf:resource="http://purl.obolibrary.org/obo/GAZ_00031093"/>
        <obo:IAO_0000115>One of the 105 woredas in the Amhara Region of Ethiopia. Part of the Semien Shewa Zone, Antsokiyana Gemza is bordered on the south by Efratana Gidim, on the west by Geshe Rabel, and on the north and east by the Oromia Region. The administrative center of this woreda is Mekoy; other towns in Antsokiyana Gemza include Majete.</obo:IAO_0000115>
        <oboInOwl:hasOBONamespace>GAZ</oboInOwl:hasOBONamespace>
        <oboInOwl:id>GAZ:00123510</oboInOwl:id>
        <rdfs:label>Antsokiyana Gemza Woreda</rdfs:label>
    </owl:NamedIndividual>
    


    <!-- http://purl.obolibrary.org/obo/GAZ_00123511 -->

    <owl:NamedIndividual rdf:about="http://purl.obolibrary.org/obo/GAZ_00123511">
        <obo:RO_0001025 rdf:resource="http://purl.obolibrary.org/obo/GAZ_00031093"/>
        <obo:IAO_0000115>One of the 105 woredas in the Amhara Region of Ethiopia. Located at the southern end of the Semien Shewa Zone, Minjjarna Shenkora is bordered on the east, south and west by the Oromia Region, on the northwest by Hagere Mariamna Kesem, and on the northeast by Berehet; the Germama River forms the boundary between this woreda and Hagere Mariamna Kesem and Berehet. The administrative center of this woreda is Balchi; other towns in the woreda include Arerti and Eranbuti.</obo:IAO_0000115>
        <oboInOwl:hasOBONamespace>GAZ</oboInOwl:hasOBONamespace>
        <oboInOwl:id>GAZ:00123511</oboInOwl:id>
        <rdfs:label>Menjarna Shenkora Woreda</rdfs:label>
    </owl:NamedIndividual>
    


    <!-- http://purl.obolibrary.org/obo/GAZ_00123512 -->

    <owl:NamedIndividual rdf:about="http://purl.obolibrary.org/obo/GAZ_00123512">
        <obo:RO_0001025 rdf:resource="http://purl.obolibrary.org/obo/GAZ_00031093"/>
        <obo:IAO_0000115>One of the 105 woredas in the Amhara Region of Ethiopia. Part of the Semien Shewa Zone, Siyadebrina Wayu Ensaro is bordered on the south and west by the Oromia Region, on the northwest by the Jamma River which separates it from Lay Betna Tach Bet, on the north by Moretna Jiru, and on the east by Debre Berhan Zuria. Towns and cities in Siyadebrina Wayu Ensaro include Ensadeneba and Lemi.</obo:IAO_0000115>
        <oboInOwl:hasOBONamespace>GAZ</oboInOwl:hasOBONamespace>
        <oboInOwl:id>GAZ:00123512</oboInOwl:id>
        <rdfs:label>Siyadebrina Wayu Ensaro Woreda</rdfs:label>
    </owl:NamedIndividual>
    


    <!-- http://purl.obolibrary.org/obo/GAZ_00123513 -->

    <owl:NamedIndividual rdf:about="http://purl.obolibrary.org/obo/GAZ_00123513">
        <obo:RO_0001025 rdf:resource="http://purl.obolibrary.org/obo/GAZ_00031093"/>
        <obo:IAO_0000115>One of the 105 woredas in the Amhara Region of Ethiopia. Part of the Semien Shewa Zone, Kewet is bordered on the southwest by Mafud Mezezo Mojana, on the northwest by Mam Midrina Lalo Midir, on the north by Efratana Gidim, and on the east and south by Afar Region. The major town in Kewet is Shewa Robit.</obo:IAO_0000115>
        <oboInOwl:hasOBONamespace>GAZ</oboInOwl:hasOBONamespace>
        <oboInOwl:id>GAZ:00123513</oboInOwl:id>
        <rdfs:label>Kewet Woreda</rdfs:label>
    </owl:NamedIndividual>
    


    <!-- http://purl.obolibrary.org/obo/GAZ_00123514 -->

    <owl:NamedIndividual rdf:about="http://purl.obolibrary.org/obo/GAZ_00123514">
        <obo:RO_0001025 rdf:resource="http://purl.obolibrary.org/obo/GAZ_00031093"/>
        <obo:IAO_0000115>One of the 105 woredas in the Amhara Region of Ethiopia. Part of the Semien Shewa Zone, Efratana Gidim is bordered on the south by Kewet, on the southwest by Mam Midrina Lalo Midir, on the west by Gera Midira Keya Gebriel, on the north by Antsokiyana Gemza, and on the east by the Oromia Zone. The administrative center of this woreda is Ataye (Efeson); other towns in Efratana Gidim include Jewha and Karakore.</obo:IAO_0000115>
        <oboInOwl:hasOBONamespace>GAZ</oboInOwl:hasOBONamespace>
        <oboInOwl:id>GAZ:00123514</oboInOwl:id>
        <rdfs:label>Efratana Gidim Woreda</rdfs:label>
    </owl:NamedIndividual>
    


    <!-- http://purl.obolibrary.org/obo/GAZ_00123515 -->

    <owl:NamedIndividual rdf:about="http://purl.obolibrary.org/obo/GAZ_00123515">
        <obo:RO_0001025 rdf:resource="http://purl.obolibrary.org/obo/GAZ_00031093"/>
        <obo:IAO_0000115>One of the 105 woredas in the Amhara Region of Ethiopia. Located at the eastern edge of the Ethiopian highlands in the Semien Shewa Zone, Angolalla Terana Asagirt is bordered on the southwest by Hagere Mariamna Kesem, on the west by the Oromia Region, on the north by Debre Berhan Zuria, on the northeast by Ankober, and on the southeast by Berehet. The administrative center of this woreda is Chacha; other towns include Choki and Gina Ager.</obo:IAO_0000115>
        <oboInOwl:hasOBONamespace>GAZ</oboInOwl:hasOBONamespace>
        <oboInOwl:id>GAZ:00123515</oboInOwl:id>
        <rdfs:label>Angolalla Terana Asagirt Woreda</rdfs:label>
    </owl:NamedIndividual>
    


    <!-- http://purl.obolibrary.org/obo/GAZ_00123516 -->

    <owl:NamedIndividual rdf:about="http://purl.obolibrary.org/obo/GAZ_00123516">
        <obo:RO_0001025 rdf:resource="http://purl.obolibrary.org/obo/GAZ_00031093"/>
        <obo:IAO_0000115>One of the 105 woredas in the Amhara Region of Ethiopia. Located at the eastern edge of the Ethiopian highlands in the Semien Shewa Zone, Mam Midrina Lalo Midir is bordered on the south by Mafud Mezezo Mojana, on the west and north by Gera Midira Keya Gebriel, on the northeast by Efratana Gidim, and on the east by Kewet.</obo:IAO_0000115>
        <oboInOwl:hasOBONamespace>GAZ</oboInOwl:hasOBONamespace>
        <oboInOwl:id>GAZ:00123516</oboInOwl:id>
        <rdfs:label>Mam Midrina Lalo Midir Woreda Woreda</rdfs:label>
    </owl:NamedIndividual>
    


    <!-- http://purl.obolibrary.org/obo/GAZ_00123517 -->

    <owl:NamedIndividual rdf:about="http://purl.obolibrary.org/obo/GAZ_00123517">
        <obo:RO_0001025 rdf:resource="http://purl.obolibrary.org/obo/GAZ_00031093"/>
        <obo:IAO_0000115>One of the 105 woredas in the Amhara Region of Ethiopia. Located at the eastern edge of the Ethiopian highlands in the Semien Shewa Zone, Gera Midira Keya Gebriel is bordered on the south by Mam Midrina Lalo Midir, on the southwest by the Jamma River which separates it from Moretna Jiru, on the northwest by the Qechene River which separates it from the Debub Wollo Zone, on the north by Geshe Rabel, and on the east by the Oromia Zone. The administrative center of this woreda is Mehal Meda; other towns include Zemero.</obo:IAO_0000115>
        <oboInOwl:hasOBONamespace>GAZ</oboInOwl:hasOBONamespace>
        <oboInOwl:id>GAZ:00123517</oboInOwl:id>
        <rdfs:label>Gera Midira Keya Gebriel Woreda</rdfs:label>
    </owl:NamedIndividual>
    


    <!-- http://purl.obolibrary.org/obo/GAZ_00123518 -->

    <owl:NamedIndividual rdf:about="http://purl.obolibrary.org/obo/GAZ_00123518">
        <obo:RO_0001025 rdf:resource="http://purl.obolibrary.org/obo/GAZ_00031093"/>
        <obo:IAO_0000115>One of the 105 woredas in the Amhara Region of Ethiopia. Located at the eastern edge of the Ethiopian highlands in the Semien Shewa Zone, Geshe Rabel is bordered on the south by the Gera Midira Keya Gebriel, on the west and north by the Debub Wollo Zone, and on the east by Antsokiyana Gemza. The administrative center of Geshe Rabel is Rabel.</obo:IAO_0000115>
        <oboInOwl:hasOBONamespace>GAZ</oboInOwl:hasOBONamespace>
        <oboInOwl:id>GAZ:00123518</oboInOwl:id>
        <rdfs:label>Geshe Rabel Woreda</rdfs:label>
    </owl:NamedIndividual>
    


    <!-- http://purl.obolibrary.org/obo/GAZ_00123519 -->

    <owl:NamedIndividual rdf:about="http://purl.obolibrary.org/obo/GAZ_00123519">
        <obo:RO_0001025 rdf:resource="http://purl.obolibrary.org/obo/GAZ_00031093"/>
        <obo:IAO_0000115>One of the 105 woredas in the Amhara Region of Ethiopia. Part of the Semien Shewa Zone, Lay Betna Tach Bet is bordered on the south by Siyadebrina Wayu Ensaro, on the west by the Oromia Region, on the north by Weremo Wajetuna Midarema, on the northeast by Gera Midira Keya Gebriel, and on the east by Moretna Jiru. The Jamma River defines this woreda&apos;s southern and eastern boundaries, and its tributary the Qechene defines its western and northern. The administrative center is Alem Ketema; other towns in this woreda include Fetira.</obo:IAO_0000115>
        <oboInOwl:hasOBONamespace>GAZ</oboInOwl:hasOBONamespace>
        <oboInOwl:id>GAZ:00123519</oboInOwl:id>
        <rdfs:label>Lay Betna Tach Bet Woreda</rdfs:label>
    </owl:NamedIndividual>
    


    <!-- http://purl.obolibrary.org/obo/GAZ_00123520 -->

    <owl:NamedIndividual rdf:about="http://purl.obolibrary.org/obo/GAZ_00123520">
        <obo:RO_0001025 rdf:resource="http://purl.obolibrary.org/obo/GAZ_00031093"/>
        <obo:IAO_0000115>One of the 105 woredas in the Amhara Region of Ethiopia. Part of the Semien Shewa Zone, Moretna Jiru is bordered on the south by Siyadebrina Wayu Ensaro, on the west by Lay Betna Tach Bet, on the north by Gera Midira Keya Gebriel, and on the east by Debre Berhan Zuria. The administrative center is Enewari.</obo:IAO_0000115>
        <oboInOwl:hasOBONamespace>GAZ</oboInOwl:hasOBONamespace>
        <oboInOwl:id>GAZ:00123520</oboInOwl:id>
        <rdfs:label>Moretna Jiru Woreda</rdfs:label>
    </owl:NamedIndividual>
    


    <!-- http://purl.obolibrary.org/obo/GAZ_00123521 -->

    <owl:NamedIndividual rdf:about="http://purl.obolibrary.org/obo/GAZ_00123521">
        <obo:RO_0001025 rdf:resource="http://purl.obolibrary.org/obo/GAZ_00031101"/>
        <obo:IAO_0000115>One of the 105 woredas in the Amhara Region of Ethiopia. Part of the Semien Wollo Zone, Habru is bordered on the south by the Debub Wollo Zone, on the west by Guba Lafto, on the north by Kobo, and on the east by the Afar Region. Towns and cities in Habru include Mersa and Wurgesa.</obo:IAO_0000115>
        <oboInOwl:hasOBONamespace>GAZ</oboInOwl:hasOBONamespace>
        <oboInOwl:id>GAZ:00123521</oboInOwl:id>
        <rdfs:label>Habru Woreda</rdfs:label>
    </owl:NamedIndividual>
    


    <!-- http://purl.obolibrary.org/obo/GAZ_00123522 -->

    <owl:NamedIndividual rdf:about="http://purl.obolibrary.org/obo/GAZ_00123522">
        <obo:RO_0001025 rdf:resource="http://purl.obolibrary.org/obo/GAZ_00031101"/>
        <obo:IAO_0000115>A woreda in northern Ethiopia. Located north of Dessie and southeast of Lalibela in the Semien Wollo Zone of the Amhara Region.</obo:IAO_0000115>
        <oboInOwl:hasOBONamespace>GAZ</oboInOwl:hasOBONamespace>
        <oboInOwl:id>GAZ:00123522</oboInOwl:id>
        <rdfs:label>Weldiya Woreda</rdfs:label>
    </owl:NamedIndividual>
    


    <!-- http://purl.obolibrary.org/obo/GAZ_00123523 -->

    <owl:NamedIndividual rdf:about="http://purl.obolibrary.org/obo/GAZ_00123523">
        <obo:RO_0001025 rdf:resource="http://purl.obolibrary.org/obo/GAZ_00031101"/>
        <obo:IAO_0000115>One of the 105 woredas in the Amhara Region of Ethiopia; it is named for the former district which lay roughly in the same area. Part of the Semien Wollo Zone, Wadla is bordered on the south and east by Dawuntna Delant, on the west by the Debub Gondar Zone, and on the north by Meket. The major town in Wadla is Kone.</obo:IAO_0000115>
        <oboInOwl:hasOBONamespace>GAZ</oboInOwl:hasOBONamespace>
        <oboInOwl:id>GAZ:00123523</oboInOwl:id>
        <rdfs:label>Wadla Woreda</rdfs:label>
    </owl:NamedIndividual>
    


    <!-- http://purl.obolibrary.org/obo/GAZ_00123524 -->

    <owl:NamedIndividual rdf:about="http://purl.obolibrary.org/obo/GAZ_00123524">
        <obo:RO_0001025 rdf:resource="http://purl.obolibrary.org/obo/GAZ_00031101"/>
        <obo:IAO_0000115>One of the 105 woredas in the Amhara Region of Ethiopia. Part of the Semien Wollo Zone, Meket is bordered on the south by Wadla, on the west by the Debub Gondar Zone, on the north by Bugna, and on the east by Guba Lafto. The major town in Meket is Filakit Gereger.</obo:IAO_0000115>
        <oboInOwl:hasOBONamespace>GAZ</oboInOwl:hasOBONamespace>
        <oboInOwl:id>GAZ:00123524</oboInOwl:id>
        <rdfs:label>Meket Woreda</rdfs:label>
    </owl:NamedIndividual>
    


    <!-- http://purl.obolibrary.org/obo/GAZ_00123525 -->

    <owl:NamedIndividual rdf:about="http://purl.obolibrary.org/obo/GAZ_00123525">
        <obo:RO_0001025 rdf:resource="http://purl.obolibrary.org/obo/GAZ_00031101"/>
        <obo:IAO_0000115>One of the 105 woredas in the Amhara Region of Ethiopia. Part of the Semien Wollo Zone, Kobo is bordered on the south by Guba Lafto, on the west by Gidan, and on the north and east by the Afar Region. Towns in Kobo include Gobiye, Kobo and Robit.</obo:IAO_0000115>
        <oboInOwl:hasOBONamespace>GAZ</oboInOwl:hasOBONamespace>
        <oboInOwl:id>GAZ:00123525</oboInOwl:id>
        <rdfs:label>Kobo Woreda</rdfs:label>
    </owl:NamedIndividual>
    


    <!-- http://purl.obolibrary.org/obo/GAZ_00123526 -->

    <owl:NamedIndividual rdf:about="http://purl.obolibrary.org/obo/GAZ_00123526">
        <obo:RO_0001025 rdf:resource="http://purl.obolibrary.org/obo/GAZ_00031101"/>
        <obo:IAO_0000115>One of the 105 woredas in the Amhara Region of Ethiopia. Part of the Semien Wollo Zone, Guba Lafto is bordered on the south by the Debub Wollo Zone, on the west by Dawuntna Delant, on the northwest by Meket, on the north by Gidan, on the northeast by Kobo, on the east by the Afar Region, and on the southeast by Habru.</obo:IAO_0000115>
        <oboInOwl:hasOBONamespace>GAZ</oboInOwl:hasOBONamespace>
        <oboInOwl:id>GAZ:00123526</oboInOwl:id>
        <rdfs:label>Guba Lafto Woreda</rdfs:label>
    </owl:NamedIndividual>
    


    <!-- http://purl.obolibrary.org/obo/GAZ_00123527 -->

    <owl:NamedIndividual rdf:about="http://purl.obolibrary.org/obo/GAZ_00123527">
        <obo:RO_0001025 rdf:resource="http://purl.obolibrary.org/obo/GAZ_00031101"/>
        <obo:IAO_0000115>One of the 105 woredas in the Amhara Region of Ethiopia. Part of the Semien Wollo Zone, Dawuntna Delant is bordered on the south by the Debub Wollo Zone, on the west by the Debub Gondar Zone, on the north by Wadla, and on the east by Guba Lafto.</obo:IAO_0000115>
        <oboInOwl:hasOBONamespace>GAZ</oboInOwl:hasOBONamespace>
        <oboInOwl:id>GAZ:00123527</oboInOwl:id>
        <rdfs:label>Dawuntna Delant Woreda</rdfs:label>
    </owl:NamedIndividual>
    


    <!-- http://purl.obolibrary.org/obo/GAZ_00123528 -->

    <owl:NamedIndividual rdf:about="http://purl.obolibrary.org/obo/GAZ_00123528">
        <obo:RO_0001025 rdf:resource="http://purl.obolibrary.org/obo/GAZ_00031101"/>
        <obo:IAO_0000115>One of the 105 woredas in the Amhara Region of Ethiopia. Part of the Semien Wollo Zone, Gidan is bordered on the south by Guba Lafto, on the southwest by Meket, on the west by Bugna, on the north by the Afar Region, and on the east by Kobo. Towns in Gidan include Debre Tsehay and Muja.</obo:IAO_0000115>
        <oboInOwl:hasOBONamespace>GAZ</oboInOwl:hasOBONamespace>
        <oboInOwl:id>GAZ:00123528</oboInOwl:id>
        <rdfs:label>Gidan Woreda</rdfs:label>
    </owl:NamedIndividual>
    


    <!-- http://purl.obolibrary.org/obo/GAZ_00123529 -->

    <owl:NamedIndividual rdf:about="http://purl.obolibrary.org/obo/GAZ_00123529">
        <obo:RO_0001025 rdf:resource="http://purl.obolibrary.org/obo/GAZ_00031099"/>
        <obo:IAO_0000115>One of the 105 woredas in the Amhara Region of Ethiopia. Part of the Semien Gondar Zone, Metemma is bordered on the south by Qwara, on the west by Sudan, on the north by Sanja, and on the east by Chilga. Towns in Metemma include Metemma, Shehedi and Shinfa.</obo:IAO_0000115>
        <oboInOwl:hasOBONamespace>GAZ</oboInOwl:hasOBONamespace>
        <oboInOwl:id>GAZ:00123529</oboInOwl:id>
        <rdfs:label>Metemma Woreda</rdfs:label>
    </owl:NamedIndividual>
    


    <!-- http://purl.obolibrary.org/obo/GAZ_00123530 -->

    <owl:NamedIndividual rdf:about="http://purl.obolibrary.org/obo/GAZ_00123530">
        <obo:RO_0001025 rdf:resource="http://purl.obolibrary.org/obo/GAZ_00031099"/>
        <obo:IAO_0000115>One of the 105 woredas in the Amhara Region of Ethiopia. Wegera is named for the former province Wegera, which was located roughly in the same location, and was later made part of the province of Semien. Part of the Semien Gondar Zone, Wegera is bordered on the south by Belessa, on the southwest by Gondar Zuria, on the west by Lay Armachiho, on the northwest by Sanja, on the north by Dabat, and on the east by Jan Amora. Towns in Wegera include Amba Giyorgis and Gedegbe.</obo:IAO_0000115>
        <oboInOwl:hasOBONamespace>GAZ</oboInOwl:hasOBONamespace>
        <oboInOwl:id>GAZ:00123530</oboInOwl:id>
        <rdfs:label>Wegera Woreda</rdfs:label>
    </owl:NamedIndividual>
    


    <!-- http://purl.obolibrary.org/obo/GAZ_00123531 -->

    <owl:NamedIndividual rdf:about="http://purl.obolibrary.org/obo/GAZ_00123531">
        <obo:RO_0001025 rdf:resource="http://purl.obolibrary.org/obo/GAZ_00031099"/>
        <obo:IAO_0000115>One of the 105 woredas in the Amhara Region of Ethiopia. Part of the Semien Gondar Zone, Sanja is bordered on the south by Chilga, on the southwest by Metemma, on the west by Sudan, on the north by the Tigray Region, on the northeast by Debarq, on the east by Dabat, and on the southeast by Wegera and Lay Armachiho. Towns in Sanja include Abderafi and Kirakir.</obo:IAO_0000115>
        <oboInOwl:hasOBONamespace>GAZ</oboInOwl:hasOBONamespace>
        <oboInOwl:id>GAZ:00123531</oboInOwl:id>
        <rdfs:label>Sanja Woreda</rdfs:label>
    </owl:NamedIndividual>
    


    <!-- http://purl.obolibrary.org/obo/GAZ_00123532 -->

    <owl:NamedIndividual rdf:about="http://purl.obolibrary.org/obo/GAZ_00123532">
        <obo:RO_0001025 rdf:resource="http://purl.obolibrary.org/obo/GAZ_00031099"/>
        <obo:IAO_0000115>One of the 105 woredas in the Amhara Region of Ethiopia. Part of the Semien Gondar Zone, Jan Amora is bordered on the south by Belessa, on the southwest by Wegera, on the west by Debarq, on the north by Addi Arkay, and on the east by Beyeda. The major town in Jan Amora is Mekane Berhan.</obo:IAO_0000115>
        <oboInOwl:hasOBONamespace>GAZ</oboInOwl:hasOBONamespace>
        <oboInOwl:id>GAZ:00123532</oboInOwl:id>
        <rdfs:label>Jan Amora Woreda</rdfs:label>
    </owl:NamedIndividual>
    


    <!-- http://purl.obolibrary.org/obo/GAZ_00123533 -->

    <owl:NamedIndividual rdf:about="http://purl.obolibrary.org/obo/GAZ_00123533">
        <obo:RO_0001025 rdf:resource="http://purl.obolibrary.org/obo/GAZ_00031099"/>
        <obo:IAO_0000115>One of the 105 woredas in the Amhara Region of Ethiopia. Part of the Semien Gondar Zone, Belessa is bordered on the south by the Debub Gondar Zone, on the west by Gondar Zuria, on the northwest by Wegera, on the northeast by Jan Amora, and on the east by the Wag Hemra Zone. Towns in Belessa include Arbaya and Hamusit.</obo:IAO_0000115>
        <oboInOwl:hasOBONamespace>GAZ</oboInOwl:hasOBONamespace>
        <oboInOwl:id>GAZ:00123533</oboInOwl:id>
        <rdfs:label>Belessa Woreda</rdfs:label>
    </owl:NamedIndividual>
    


    <!-- http://purl.obolibrary.org/obo/GAZ_00123534 -->

    <owl:NamedIndividual rdf:about="http://purl.obolibrary.org/obo/GAZ_00123534">
        <obo:RO_0001025 rdf:resource="http://purl.obolibrary.org/obo/GAZ_00031099"/>
        <obo:IAO_0000115>One of the 105 woredas in the Amhara Region of Ethiopia. It is named after its largest town, Debarq. Part of the Semien Gondar Zone, Debarq is bordered on the south by Dabat, on the west by Sanja, on the northwest by the Tigray Region, on the north by Addi Arkay, and on the east by Jan Amora.</obo:IAO_0000115>
        <oboInOwl:hasOBONamespace>GAZ</oboInOwl:hasOBONamespace>
        <oboInOwl:id>GAZ:00123534</oboInOwl:id>
        <rdfs:label>Debarq Woreda</rdfs:label>
    </owl:NamedIndividual>
    


    <!-- http://purl.obolibrary.org/obo/GAZ_00123535 -->

    <owl:NamedIndividual rdf:about="http://purl.obolibrary.org/obo/GAZ_00123535">
        <obo:RO_0001025 rdf:resource="http://purl.obolibrary.org/obo/GAZ_00031099"/>
        <obo:IAO_0000115>One of the 105 woredas in the Amhara Region of Ethiopia. Part of the Semien Gondar Zone, Addi Arkay is bordered on the south by Jan Amora, on the southwest by Debarq, on the north and east by the Tigray Region, and on the southeast by Beyeda; its eastern border is defined by the Tekeze River. Towns in Addi Arkay include Addi Arkay and Zarima.</obo:IAO_0000115>
        <oboInOwl:hasOBONamespace>GAZ</oboInOwl:hasOBONamespace>
        <oboInOwl:id>GAZ:00123535</oboInOwl:id>
        <rdfs:label>Addi Arkay Woreda</rdfs:label>
    </owl:NamedIndividual>
    


    <!-- http://purl.obolibrary.org/obo/GAZ_00123536 -->

    <owl:NamedIndividual rdf:about="http://purl.obolibrary.org/obo/GAZ_00123536">
        <obo:RO_0001025 rdf:resource="http://purl.obolibrary.org/obo/GAZ_00031099"/>
        <obo:IAO_0000115>One of the 105 woredas in the Amhara Region of Ethiopia. It is named after its chief town Chilga (also known as Ayikel), an important stopping point on the historic Gondar-Sudan trade route. Part of the Semien Gondar Zone, Chilga is bordered on the south by Alefa, on the west by Metemma, on the north by Sanja, on the northeast by Lay Armachiho, and on the east by Dembiya. Other towns in Chilga include Seraba.</obo:IAO_0000115>
        <oboInOwl:hasOBONamespace>GAZ</oboInOwl:hasOBONamespace>
        <oboInOwl:id>GAZ:00123536</oboInOwl:id>
        <rdfs:label>Chilga Woreda</rdfs:label>
    </owl:NamedIndividual>
    


    <!-- http://purl.obolibrary.org/obo/GAZ_00123537 -->

    <owl:NamedIndividual rdf:about="http://purl.obolibrary.org/obo/GAZ_00123537">
        <obo:RO_0001025 rdf:resource="http://purl.obolibrary.org/obo/GAZ_00031099"/>
        <obo:IAO_0000115>One of the 105 woredas in the Amhara Region of Ethiopia. Part of the Semien Gondar Zone, Lay Armachiho is bordered on the south by Dembiya, on the west by Chilga, on the north by Sanja, on the east by Wegera, and on the southeast by Gondar Zuria. The major town in Lay Armachiho is Tekle Dingay.</obo:IAO_0000115>
        <oboInOwl:hasOBONamespace>GAZ</oboInOwl:hasOBONamespace>
        <oboInOwl:id>GAZ:00123537</oboInOwl:id>
        <rdfs:label>Lay Armachiho Woreda</rdfs:label>
    </owl:NamedIndividual>
    


    <!-- http://purl.obolibrary.org/obo/GAZ_00123538 -->

    <owl:NamedIndividual rdf:about="http://purl.obolibrary.org/obo/GAZ_00123538">
        <obo:RO_0001025 rdf:resource="http://purl.obolibrary.org/obo/GAZ_00031099"/>
        <obo:IAO_0000115>One of the 105 woredas in the Amhara Region of Ethiopia. Part of the Semien Gondar Zone, Alefa is bordered on the south by the Benishangul-Gumuz Region, on the west by Qwara, on the northwest by Metemma, on the north by Chilga, on the northeast by Dembiya, and on the east by Lake Tana. The capital of Alefa is Shawra; other towns include Delgi, Dengel Ber, Esey Dibir and Gomenge. Rivers include the Dinder.</obo:IAO_0000115>
        <oboInOwl:hasOBONamespace>GAZ</oboInOwl:hasOBONamespace>
        <oboInOwl:id>GAZ:00123538</oboInOwl:id>
        <rdfs:label>Alefa Woreda</rdfs:label>
    </owl:NamedIndividual>
    


    <!-- http://purl.obolibrary.org/obo/GAZ_00123539 -->

    <owl:NamedIndividual rdf:about="http://purl.obolibrary.org/obo/GAZ_00123539">
        <obo:RO_0001025 rdf:resource="http://purl.obolibrary.org/obo/GAZ_00031099"/>
        <obo:IAO_0000115>One of the 105 woredas in the Amhara Region of Ethiopia. Part of the Semien Gondar Zone, Beyeda is bordered on the south by the Wag Hemra Zone, on the west by Jan Amora, on the north by Addi Arkay, and on the east by the Tekeze River which separates it from the Tigray Region. The major town in Beyeda is Dilyibza.</obo:IAO_0000115>
        <oboInOwl:hasOBONamespace>GAZ</oboInOwl:hasOBONamespace>
        <oboInOwl:id>GAZ:00123539</oboInOwl:id>
        <rdfs:label>Beyeda Woreda</rdfs:label>
    </owl:NamedIndividual>
    


    <!-- http://purl.obolibrary.org/obo/GAZ_00123540 -->

    <owl:NamedIndividual rdf:about="http://purl.obolibrary.org/obo/GAZ_00123540">
        <obo:RO_0001025 rdf:resource="http://purl.obolibrary.org/obo/GAZ_00031099"/>
        <obo:IAO_0000115>One of the 105 woredas in the Amhara Region of Ethiopia. Part of the Semien Gondar Zone, Dabat is bordered on the south by Wegera, on the west by Sanja, and on the northeast by Debarq. Towns in Dabat include Dabat and Wekin.</obo:IAO_0000115>
        <oboInOwl:hasOBONamespace>GAZ</oboInOwl:hasOBONamespace>
        <oboInOwl:id>GAZ:00123540</oboInOwl:id>
        <rdfs:label>Dabat Woreda</rdfs:label>
    </owl:NamedIndividual>
    


    <!-- http://purl.obolibrary.org/obo/GAZ_00123541 -->

    <owl:NamedIndividual rdf:about="http://purl.obolibrary.org/obo/GAZ_00123541">
        <obo:RO_0001025 rdf:resource="http://purl.obolibrary.org/obo/GAZ_00031099"/>
        <obo:IAO_0000115>One of the 105 woredas in the Amhara Region of Ethiopia. Part of the Semien Gondar Zone, Dembiya is bordered on the south by Lake Tana, on the southwest by Alefa, on the west by Chilga, on the north by Lay Armachiho, and on the east by Gondar Zuria. Towns in Dembiya include Aymiba, Chuahit, Gorgora and Koladiba.</obo:IAO_0000115>
        <oboInOwl:hasOBONamespace>GAZ</oboInOwl:hasOBONamespace>
        <oboInOwl:id>GAZ:00123541</oboInOwl:id>
        <rdfs:label>Dembiya Woreda</rdfs:label>
    </owl:NamedIndividual>
    


    <!-- http://purl.obolibrary.org/obo/GAZ_00123542 -->

    <owl:NamedIndividual rdf:about="http://purl.obolibrary.org/obo/GAZ_00123542">
        <obo:RO_0001025 rdf:resource="http://purl.obolibrary.org/obo/GAZ_00031099"/>
        <obo:IAO_0000115>One of the 105 woredas in the Amhara Region of Ethiopia. Part of the Semien Gondar Zone, Qwara is bordered on the south by the Benishangul-Gumuz Region, on the west by Sudan, on the north by Metemma, and on the east by Alefa; part of its boundary with the Benishangul-Gumaz Region is defined by the Dinder River. The administrative center of this woreda is Gelegu; other settlements include Tewodros Ketema.</obo:IAO_0000115>
        <oboInOwl:hasOBONamespace>GAZ</oboInOwl:hasOBONamespace>
        <oboInOwl:id>GAZ:00123542</oboInOwl:id>
        <rdfs:label>Qwara Woreda</rdfs:label>
    </owl:NamedIndividual>
    


    <!-- http://purl.obolibrary.org/obo/GAZ_00123543 -->

    <owl:NamedIndividual rdf:about="http://purl.obolibrary.org/obo/GAZ_00123543">
        <obo:RO_0001025 rdf:resource="http://purl.obolibrary.org/obo/GAZ_00000567"/>
        <obo:IAO_0000115>A rugged mass of mountains in Ethiopia, Eritrea (which is sometimes referred to as the Eritrean Highlands), and northern Somalia (Somaliland) in the Horn of Africa.</obo:IAO_0000115>
        <oboInOwl:hasOBONamespace>GAZ</oboInOwl:hasOBONamespace>
        <oboInOwl:id>GAZ:00123543</oboInOwl:id>
        <rdfs:label>Ethiopian Highlands</rdfs:label>
    </owl:NamedIndividual>
    


    <!-- http://purl.obolibrary.org/obo/GAZ_00123544 -->

    <owl:NamedIndividual rdf:about="http://purl.obolibrary.org/obo/GAZ_00123544">
        <obo:RO_0001025 rdf:resource="http://purl.obolibrary.org/obo/GAZ_00123543"/>
        <obo:IAO_0000115>An extension of the Ethiopian Highlands to the south. The Eritrean Highlands are drained by four major rivers towards Sudan and by several smaller rivers into the Red Sea coast of Eritrea. Flowing towards Sudan and the Nile River are the Gash and Setit Rivers while towards Sudan without reaching the Nile are the Barka and Anseba Rivers. The Eastern Escarpment of Eritrea is drained by numerous small streams.</obo:IAO_0000115>
        <oboInOwl:hasOBONamespace>GAZ</oboInOwl:hasOBONamespace>
        <oboInOwl:id>GAZ:00123544</oboInOwl:id>
        <rdfs:label>Eritrean Highlands</rdfs:label>
    </owl:NamedIndividual>
    


    <!-- http://purl.obolibrary.org/obo/GAZ_00123545 -->

    <owl:NamedIndividual rdf:about="http://purl.obolibrary.org/obo/GAZ_00123545">
        <obo:RO_0001025 rdf:resource="http://purl.obolibrary.org/obo/GAZ_00031093"/>
        <obo:IAO_0000115>One of the 105 woredas in the Amhara Region of Ethiopia. Located at the eastern edge of the Ethiopian highlands in the Semien Shewa Zone, Debre Berhan Zuria is bordered on the south by Angolalla Terana Asagirt, on the southwest by Siyadebrina Wayu Ensaro, on the northwest by Moretna Jiru, on the north by Mafud Mezezo Mojana, and on the east by Ankober. The town and woreda of Debre Berhan is an enclave inside this woreda.</obo:IAO_0000115>
        <oboInOwl:hasOBONamespace>GAZ</oboInOwl:hasOBONamespace>
        <oboInOwl:id>GAZ:00123545</oboInOwl:id>
        <rdfs:label>Debre Berhan Zuria Woreda</rdfs:label>
    </owl:NamedIndividual>
    


    <!-- http://purl.obolibrary.org/obo/GAZ_00123546 -->

    <owl:NamedIndividual rdf:about="http://purl.obolibrary.org/obo/GAZ_00123546">
        <obo:RO_0001025 rdf:resource="http://purl.obolibrary.org/obo/GAZ_00000781"/>
        <obo:IAO_0000115>One of the 21 woredas in the Benishangul-Gumuz Region of Ethiopia. Because Pawe is not part of any Zone in Benishangul-Gumuz, it is considered a Special woreda. Pawe is bordered on the south and west by Metekel, and on the east and north by the Amhara Region. The largest town in Pawe is Almu.</obo:IAO_0000115>
        <oboInOwl:hasOBONamespace>GAZ</oboInOwl:hasOBONamespace>
        <oboInOwl:id>GAZ:00123546</oboInOwl:id>
        <rdfs:label>Pawe Special Woreda</rdfs:label>
    </owl:NamedIndividual>
    


    <!-- http://purl.obolibrary.org/obo/GAZ_00123547 -->

    <owl:NamedIndividual rdf:about="http://purl.obolibrary.org/obo/GAZ_00123547">
        <obo:RO_0001025 rdf:resource="http://purl.obolibrary.org/obo/GAZ_00031105"/>
        <obo:IAO_0000115>One of the 21 woredas in the Benishangul-Gumuz Region of Ethiopia. It is named after its highest point, Mount Bulen. Part of the Metekel Zone, Bulen is bordered by Dangur in the north, by Mandura in the northeast, by Dibate in the east, by the Abay River on the south which separates it from the Kamashi Zone, and by Wenbera in the west. Its largest settlement is Bulen.</obo:IAO_0000115>
        <oboInOwl:hasOBONamespace>GAZ</oboInOwl:hasOBONamespace>
        <oboInOwl:id>GAZ:00123547</oboInOwl:id>
        <rdfs:label>Bulen Woreda</rdfs:label>
    </owl:NamedIndividual>
    


    <!-- http://purl.obolibrary.org/obo/GAZ_00123548 -->

    <owl:NamedIndividual rdf:about="http://purl.obolibrary.org/obo/GAZ_00123548">
        <obo:RO_0001025 rdf:resource="http://purl.obolibrary.org/obo/GAZ_00031105"/>
        <obo:IAO_0000115>One of the 21 woredas in the Benishangul-Gumuz Region of Ethiopia. Part of the Metekel Zone, Guba is bordered by the Abay River on the south which separates it from the Asosa Zone, Sudan on the west, Dangur on the north and east, and on the southeast by the Beles River which separates it from Wenbera. Towns in Guba include Mankush.</obo:IAO_0000115>
        <oboInOwl:hasOBONamespace>GAZ</oboInOwl:hasOBONamespace>
        <oboInOwl:id>GAZ:00123548</oboInOwl:id>
        <rdfs:label>Guba Woreda</rdfs:label>
    </owl:NamedIndividual>
    


    <!-- http://purl.obolibrary.org/obo/GAZ_00123549 -->

    <owl:NamedIndividual rdf:about="http://purl.obolibrary.org/obo/GAZ_00123549">
        <obo:RO_0001025 rdf:resource="http://purl.obolibrary.org/obo/GAZ_00031105"/>
        <obo:IAO_0000115>One of the 21 woredas in the Benishangul-Gumuz Region of Ethiopia. Part of the Metekel Zone, Wenbera is bordered on the south by the Kamashi Zone, on the west by the Asosa Zone, on the north by Guba, on the northeast by the Beles River which separates it from Dangur, and by Bulen on the east; the Abay River defines the boundary between Wenbera and the Asosa and Kamashi Zones.</obo:IAO_0000115>
        <oboInOwl:hasOBONamespace>GAZ</oboInOwl:hasOBONamespace>
        <oboInOwl:id>GAZ:00123549</oboInOwl:id>
        <rdfs:label>Wenbera Woreda</rdfs:label>
    </owl:NamedIndividual>
    


    <!-- http://purl.obolibrary.org/obo/GAZ_00123550 -->

    <owl:NamedIndividual rdf:about="http://purl.obolibrary.org/obo/GAZ_00123550">
        <obo:RO_0001025 rdf:resource="http://purl.obolibrary.org/obo/GAZ_00031105"/>
        <obo:IAO_0000115>One of the 21 woredas in the Benishangul-Gumuz Region of Ethiopia. The administrative center of this woreda is Manbuk. Part of the Metekel Zone, Dangur is bordered by Amhara Region in the north, by Pawe special woreda in the east, by Mandura in the southeast, by Bulen in the south, by Wenbera in the southwest, and by Guba and Sudan in the west.</obo:IAO_0000115>
        <oboInOwl:hasOBONamespace>GAZ</oboInOwl:hasOBONamespace>
        <oboInOwl:id>GAZ:00123550</oboInOwl:id>
        <rdfs:label>Dangur Woreda</rdfs:label>
    </owl:NamedIndividual>
    


    <!-- http://purl.obolibrary.org/obo/GAZ_00123551 -->

    <owl:NamedIndividual rdf:about="http://purl.obolibrary.org/obo/GAZ_00123551">
        <obo:RO_0001025 rdf:resource="http://purl.obolibrary.org/obo/GAZ_00031105"/>
        <obo:IAO_0000115>One of the 21 woredas in the Benishangul-Gumuz Region of Ethiopia. Part of the Metekel Zone, Dibate is bordered by Mandura on the north, by the Amhara Region on the east, by the Abay River on the south which separates it from the Kamashi Zone, and by Bulen on the west.</obo:IAO_0000115>
        <oboInOwl:hasOBONamespace>GAZ</oboInOwl:hasOBONamespace>
        <oboInOwl:id>GAZ:00123551</oboInOwl:id>
        <rdfs:label>Dibate Woreda</rdfs:label>
    </owl:NamedIndividual>
    


    <!-- http://purl.obolibrary.org/obo/GAZ_00123552 -->

    <owl:NamedIndividual rdf:about="http://purl.obolibrary.org/obo/GAZ_00123552">
        <obo:RO_0001025 rdf:resource="http://purl.obolibrary.org/obo/GAZ_00031105"/>
        <obo:IAO_0000115>One of the 21 woredas in the Benishangul-Gumuz Region of Ethiopia. Part of the Metekel Zone, Mandura is bordered by Dangur in the north and northwest, by Pawe special woreda in the northeast, by Amhara Region in the east, by Dibate in the south, and by Bulen in the southwest. Towns in Mandura include Genete Mariam.</obo:IAO_0000115>
        <oboInOwl:hasOBONamespace>GAZ</oboInOwl:hasOBONamespace>
        <oboInOwl:id>GAZ:00123552</oboInOwl:id>
        <rdfs:label>Mandura Woreda</rdfs:label>
    </owl:NamedIndividual>
    


    <!-- http://purl.obolibrary.org/obo/GAZ_00123553 -->

    <owl:NamedIndividual rdf:about="http://purl.obolibrary.org/obo/GAZ_00123553">
        <obo:RO_0001025 rdf:resource="http://purl.obolibrary.org/obo/GAZ_00031107"/>
        <obo:IAO_0000115>One of the 21 woredas in the Benishangul-Gumuz Region of Ethiopia. Part of the Kamashi Zone, Agalo Mite is bordered by Kamashi woreda on the southeast, by the Oromia Region on the southwest, by Sirba Abbay on the northwest, by the Abay River on the north which separates it from the Metekel Zone, and by the Didessa River on the northeast which separates it from Yaso.</obo:IAO_0000115>
        <oboInOwl:hasOBONamespace>GAZ</oboInOwl:hasOBONamespace>
        <oboInOwl:id>GAZ:00123553</oboInOwl:id>
        <rdfs:label>Agalo Mite Woreda</rdfs:label>
    </owl:NamedIndividual>
    


    <!-- http://purl.obolibrary.org/obo/GAZ_00123554 -->

    <owl:NamedIndividual rdf:about="http://purl.obolibrary.org/obo/GAZ_00123554">
        <obo:RO_0001025 rdf:resource="http://purl.obolibrary.org/obo/GAZ_00031107"/>
        <obo:IAO_0000115>One of the 21 woredas in the Benishangul-Gumuz Region of Ethiopia. Part of the Kamashi Zone, Belo Jegonfoy is bordered by Kamashi in the west, by Yaso in the north, and by Oromia Region in the south; parts of the woreda are enclaves in the Oromia Region.</obo:IAO_0000115>
        <oboInOwl:hasOBONamespace>GAZ</oboInOwl:hasOBONamespace>
        <oboInOwl:id>GAZ:00123554</oboInOwl:id>
        <rdfs:label>Belo Jegonfoy Woreda</rdfs:label>
    </owl:NamedIndividual>
    


    <!-- http://purl.obolibrary.org/obo/GAZ_00123555 -->

    <owl:NamedIndividual rdf:about="http://purl.obolibrary.org/obo/GAZ_00123555">
        <obo:RO_0001025 rdf:resource="http://purl.obolibrary.org/obo/GAZ_00031107"/>
        <obo:IAO_0000115>One of the 21 woredas in the Benishangul-Gumuz Region of Ethiopia. Part of the Kamashi Zone, Yaso is bordered by the Abay River on the north which separates it from Wenbera, Bulen, Dibate and the Amhara Region, by the Oromia Region in the southeast, by Belo Jegonfoy in the south, and by the Didessa River on the west which separates it from Kamashi and Agalo Mite.</obo:IAO_0000115>
        <oboInOwl:hasOBONamespace>GAZ</oboInOwl:hasOBONamespace>
        <oboInOwl:id>GAZ:00123555</oboInOwl:id>
        <rdfs:label>Yaso Woreda</rdfs:label>
    </owl:NamedIndividual>
    


    <!-- http://purl.obolibrary.org/obo/GAZ_00123556 -->

    <owl:NamedIndividual rdf:about="http://purl.obolibrary.org/obo/GAZ_00123556">
        <obo:RO_0001025 rdf:resource="http://purl.obolibrary.org/obo/GAZ_00031107"/>
        <obo:IAO_0000115>One of the 21 woredas in the Benishangul-Gumuz Region of Ethiopia. Part of the Kamashi Zone, Sirba Abbay is bordered by the Oromia Region on the southwest, by Oda Godere on the west, by the Dabus River on the northwest which separates it from the Asosa Zone, by the Abay River on the northeast which separates it from the Metekel Zone, and by Agalo Mite on the east and south.</obo:IAO_0000115>
        <oboInOwl:hasOBONamespace>GAZ</oboInOwl:hasOBONamespace>
        <oboInOwl:id>GAZ:00123556</oboInOwl:id>
        <rdfs:label>Sirba Abbay Woreda</rdfs:label>
    </owl:NamedIndividual>
    


    <!-- http://purl.obolibrary.org/obo/GAZ_00123557 -->

    <owl:NamedIndividual rdf:about="http://purl.obolibrary.org/obo/GAZ_00123557">
        <obo:RO_0001025 rdf:resource="http://purl.obolibrary.org/obo/GAZ_00031107"/>
        <obo:IAO_0000115>One of the 21 woredas in the Benishangul-Gumuz Region of Ethiopia. Part of the Kamashi Zone, Kamashi is bordered by the Didessa River on the northeast which separates it from Yaso, by Belo Jegonfoy in the east, by the Oromia Region on the south and west, and by Agalo Mite on the northwest.</obo:IAO_0000115>
        <oboInOwl:hasOBONamespace>GAZ</oboInOwl:hasOBONamespace>
        <oboInOwl:id>GAZ:00123557</oboInOwl:id>
        <rdfs:label>Kamashi Woreda</rdfs:label>
    </owl:NamedIndividual>
    


    <!-- http://purl.obolibrary.org/obo/GAZ_00123558 -->

    <owl:NamedIndividual rdf:about="http://purl.obolibrary.org/obo/GAZ_00123558">
        <obo:RO_0001025 rdf:resource="http://purl.obolibrary.org/obo/GAZ_00031104"/>
        <obo:IAO_0000115>One of the 21 woredas in the Benishangul-Gumuz Region of Ethiopia.</obo:IAO_0000115>
        <oboInOwl:hasOBONamespace>GAZ</oboInOwl:hasOBONamespace>
        <oboInOwl:id>GAZ:00123558</oboInOwl:id>
        <rdfs:label>Begia Woreda</rdfs:label>
    </owl:NamedIndividual>
    


    <!-- http://purl.obolibrary.org/obo/GAZ_00123559 -->

    <owl:NamedIndividual rdf:about="http://purl.obolibrary.org/obo/GAZ_00123559">
        <obo:RO_0001025 rdf:resource="http://purl.obolibrary.org/obo/GAZ_00031104"/>
        <obo:IAO_0000115>One of the 21 woredas in the Benishangul-Gumuz Region of Ethiopia. Part of the Asosa Zone, Menge is bordered by Bambasi on the south, by Asosa in the southwest, by Kormuk in the northwest, by Sherkole in the north, and by the Dabus River on the east which separates it from Oda Godere.</obo:IAO_0000115>
        <oboInOwl:hasOBONamespace>GAZ</oboInOwl:hasOBONamespace>
        <oboInOwl:id>GAZ:00123559</oboInOwl:id>
        <rdfs:label>Mengea Woreda</rdfs:label>
    </owl:NamedIndividual>
    


    <!-- http://purl.obolibrary.org/obo/GAZ_00123560 -->

    <owl:NamedIndividual rdf:about="http://purl.obolibrary.org/obo/GAZ_00123560">
        <obo:RO_0001025 rdf:resource="http://purl.obolibrary.org/obo/GAZ_00031104"/>
        <obo:IAO_0000115>One of the 21 woredas in the Benishangul-Gumuz Region of Ethiopia. Part of the Asosa Zone, Sherkole is bordered by Menge on the south, Kormuk on the southwest, by Sudan on the northwest, by the Abay River on the northeast which separates it from the Metekel Zone, and the Dabus River on the southeast which separates it from the Kamashi Zone and Oda Godere.</obo:IAO_0000115>
        <oboInOwl:hasOBONamespace>GAZ</oboInOwl:hasOBONamespace>
        <oboInOwl:id>GAZ:00123560</oboInOwl:id>
        <rdfs:label>Sherkolea Woreda</rdfs:label>
    </owl:NamedIndividual>
    


    <!-- http://purl.obolibrary.org/obo/GAZ_00123561 -->

    <owl:NamedIndividual rdf:about="http://purl.obolibrary.org/obo/GAZ_00123561">
        <obo:RO_0001025 rdf:resource="http://purl.obolibrary.org/obo/GAZ_00031104"/>
        <obo:IAO_0000115>One of the 21 woredas in the Benishangul-Gumuz Region of Ethiopia. Part of the Asosa Zone, Asosa is bordered by Kormuk in the north, by Menge in the northeast, by Bambasi in the southeast, and by Sudan in the west.</obo:IAO_0000115>
        <oboInOwl:hasOBONamespace>GAZ</oboInOwl:hasOBONamespace>
        <oboInOwl:id>GAZ:00123561</oboInOwl:id>
        <rdfs:label>Asosa Woreda</rdfs:label>
    </owl:NamedIndividual>
    


    <!-- http://purl.obolibrary.org/obo/GAZ_00123562 -->

    <owl:NamedIndividual rdf:about="http://purl.obolibrary.org/obo/GAZ_00123562">
        <obo:RO_0001025 rdf:resource="http://purl.obolibrary.org/obo/GAZ_00031104"/>
        <obo:IAO_0000115>One of the 21 woredas in the Benishangul-Gumuz Region of Ethiopia. Part of the Asosa Zone, Komesha is bordered by the Oromia Region on the south, Bambasi and Menge woredas on the west, and Sirba Abbay woreda on the north and east.</obo:IAO_0000115>
        <oboInOwl:hasOBONamespace>GAZ</oboInOwl:hasOBONamespace>
        <oboInOwl:id>GAZ:00123562</oboInOwl:id>
        <rdfs:label>Komeshaa Woreda</rdfs:label>
    </owl:NamedIndividual>
    


    <!-- http://purl.obolibrary.org/obo/GAZ_00123563 -->

    <owl:NamedIndividual rdf:about="http://purl.obolibrary.org/obo/GAZ_00123563">
        <obo:RO_0001025 rdf:resource="http://purl.obolibrary.org/obo/GAZ_00031104"/>
        <obo:IAO_0000115>One of the 21 woredas in the Benishangul-Gumuz Region of Ethiopia. Part of the Asosa Zone, Kormuk is bordered by Sudan in the north and west, by Sherkole in the east, by Menge in the southwest, and by Asosa in the south.</obo:IAO_0000115>
        <oboInOwl:hasOBONamespace>GAZ</oboInOwl:hasOBONamespace>
        <oboInOwl:id>GAZ:00123563</oboInOwl:id>
        <rdfs:label>Kormuka Woreda</rdfs:label>
    </owl:NamedIndividual>
    


    <!-- http://purl.obolibrary.org/obo/GAZ_00123564 -->

    <owl:NamedIndividual rdf:about="http://purl.obolibrary.org/obo/GAZ_00123564">
        <obo:RO_0001025 rdf:resource="http://purl.obolibrary.org/obo/GAZ_00031104"/>
        <obo:IAO_0000115>One of the 21 woredas in the Benishangul-Gumuz Region of Ethiopia. Part of the Asosa Zone, Oda Godere is bordered by Sirba Abbay in the north and east, by Oromia Region in the south, by Bambasi and Menge in the west, and by Sherkole in the north. The major settlement in this woreda is Oda Buldigilu.</obo:IAO_0000115>
        <oboInOwl:hasOBONamespace>GAZ</oboInOwl:hasOBONamespace>
        <oboInOwl:id>GAZ:00123564</oboInOwl:id>
        <rdfs:label>Oda Goderea Woreda</rdfs:label>
    </owl:NamedIndividual>
    


    <!-- http://purl.obolibrary.org/obo/GAZ_00123565 -->

    <owl:NamedIndividual rdf:about="http://purl.obolibrary.org/obo/GAZ_00123565">
        <obo:RO_0001025 rdf:resource="http://purl.obolibrary.org/obo/GAZ_00031104"/>
        <obo:IAO_0000115>One of the 21 woredas in the Benishangul-Gumuz Region of Ethiopia. Part of the Asosa Zone, Bambasi is bordered by the Mao-Komo special woreda on the southwest, Asosa in the northwest, by Menge in the north, by Oda Godere in the northeast, and by the Oromia Region in the south.</obo:IAO_0000115>
        <oboInOwl:hasOBONamespace>GAZ</oboInOwl:hasOBONamespace>
        <oboInOwl:id>GAZ:00123565</oboInOwl:id>
        <rdfs:label>Bambasia Woreda</rdfs:label>
    </owl:NamedIndividual>
    


    <!-- http://purl.obolibrary.org/obo/GAZ_00123566 -->

    <owl:NamedIndividual rdf:about="http://purl.obolibrary.org/obo/GAZ_00123566">
        <obo:RO_0001025 rdf:resource="http://purl.obolibrary.org/obo/GAZ_00123560"/>
        <obo:IAO_0000115>A refugee camp.</obo:IAO_0000115>
        <oboInOwl:hasOBONamespace>GAZ</oboInOwl:hasOBONamespace>
        <oboInOwl:id>GAZ:00123566</oboInOwl:id>
        <rdfs:label>Sherkole Refugee Camp</rdfs:label>
    </owl:NamedIndividual>
    


    <!-- http://purl.obolibrary.org/obo/GAZ_00123567 -->

    <owl:NamedIndividual rdf:about="http://purl.obolibrary.org/obo/GAZ_00123567">
        <obo:RO_0001025 rdf:resource="http://purl.obolibrary.org/obo/GAZ_00031108"/>
        <obo:IAO_0000115>One of the eight woredas in the Gambela Region of Ethiopia. Part of the Administrative Zone 1, Gambela is bordered on the south by the Administrative Zone 2, on the west by Itang, and on the north and east by the Oromia Region. The major town in Gambela is Gambela.</obo:IAO_0000115>
        <oboInOwl:hasOBONamespace>GAZ</oboInOwl:hasOBONamespace>
        <oboInOwl:id>GAZ:00123567</oboInOwl:id>
        <rdfs:label>Gambela Woreda</rdfs:label>
    </owl:NamedIndividual>
    


    <!-- http://purl.obolibrary.org/obo/GAZ_00123568 -->

    <owl:NamedIndividual rdf:about="http://purl.obolibrary.org/obo/GAZ_00123568">
        <obo:RO_0001025 rdf:resource="http://purl.obolibrary.org/obo/GAZ_00031108"/>
        <obo:IAO_0000115>One of the eight woredas in the Gambela Region of Ethiopia. Part of the Administrative Zone 1, Itang is bordered on the south by the Administrative Zone 2, on the west by Administrative Zone 3, on the north by the Oromia Region, and on the east by Gambela; part of the southern boundary is defined by the Alwero River.</obo:IAO_0000115>
        <oboInOwl:hasOBONamespace>GAZ</oboInOwl:hasOBONamespace>
        <oboInOwl:id>GAZ:00123568</oboInOwl:id>
        <rdfs:label>Itang Woreda</rdfs:label>
    </owl:NamedIndividual>
    


    <!-- http://purl.obolibrary.org/obo/GAZ_00123569 -->

    <owl:NamedIndividual rdf:about="http://purl.obolibrary.org/obo/GAZ_00123569">
        <obo:RO_0001025 rdf:resource="http://purl.obolibrary.org/obo/GAZ_00031111"/>
        <obo:IAO_0000115>One of the eight woredas in the Gambela Region of Ethiopia. Part of the Administrative Zone 2, Jor is bordered on the south by the Akobo River which separates it from Sudan, on the west and north by the Administrative Zone 3, on the northeast by Abobo, and on the east by Gog; the Alwero River defines part of its northern boundary. Information is lacking on the towns of this woreda.</obo:IAO_0000115>
        <oboInOwl:hasOBONamespace>GAZ</oboInOwl:hasOBONamespace>
        <oboInOwl:id>GAZ:00123569</oboInOwl:id>
        <rdfs:label>Jor Woreda</rdfs:label>
    </owl:NamedIndividual>
    


    <!-- http://purl.obolibrary.org/obo/GAZ_00123570 -->

    <owl:NamedIndividual rdf:about="http://purl.obolibrary.org/obo/GAZ_00123570">
        <obo:RO_0001025 rdf:resource="http://purl.obolibrary.org/obo/GAZ_00031111"/>
        <obo:IAO_0000115>One of the eight woredas in the Gambela Region of Ethiopia. Part of the Administrative Zone 2, Gog is bordered on the south by the Southern Nations, Nationalities and Peoples Region, on the southwest by Sudan, on the west by Jor, on the north by Abobo, and on the east by the Godere special woreda. The major town in Gog is Fugnido.</obo:IAO_0000115>
        <oboInOwl:hasOBONamespace>GAZ</oboInOwl:hasOBONamespace>
        <oboInOwl:id>GAZ:00123570</oboInOwl:id>
        <rdfs:label>Gog Woreda</rdfs:label>
    </owl:NamedIndividual>
    


    <!-- http://purl.obolibrary.org/obo/GAZ_00123571 -->

    <owl:NamedIndividual rdf:about="http://purl.obolibrary.org/obo/GAZ_00123571">
        <obo:RO_0001025 rdf:resource="http://purl.obolibrary.org/obo/GAZ_00031111"/>
        <obo:IAO_0000115>One of the eight woredas in the Gambela Region of Ethiopia. Part of the Administrative Zone 2, Abobo is bordered on the southwest by the Godere special woreda, on the south by Gog, on the southwest by Jor, on the west by the Administrative Zone 3, on the north by the Administrative Zone 1, and on the east by the Oromia Region; part of its northern bundary is defined by the Alwero River. The major town in Abobo is Abobo.</obo:IAO_0000115>
        <oboInOwl:hasOBONamespace>GAZ</oboInOwl:hasOBONamespace>
        <oboInOwl:id>GAZ:00123571</oboInOwl:id>
        <rdfs:label>Abobo Woreda</rdfs:label>
    </owl:NamedIndividual>
    


    <!-- http://purl.obolibrary.org/obo/GAZ_00123572 -->

    <owl:NamedIndividual rdf:about="http://purl.obolibrary.org/obo/GAZ_00123572">
        <obo:RO_0001025 rdf:resource="http://purl.obolibrary.org/obo/GAZ_00123571"/>
        <obo:IAO_0000115>A lake.</obo:IAO_0000115>
        <oboInOwl:hasOBONamespace>GAZ</oboInOwl:hasOBONamespace>
        <oboInOwl:id>GAZ:00123572</oboInOwl:id>
        <rdfs:label>Lake Alwero</rdfs:label>
    </owl:NamedIndividual>
    


    <!-- http://purl.obolibrary.org/obo/GAZ_00123573 -->

    <owl:NamedIndividual rdf:about="http://purl.obolibrary.org/obo/GAZ_00123573">
        <obo:RO_0001025 rdf:resource="http://purl.obolibrary.org/obo/GAZ_00031109"/>
        <obo:IAO_0000115>One of the eight woredas in the Gambela Region of Ethiopia. It is named after the Akobo River, which flows westwards then north into the Baro River, defining its border with Sudan. Part of the Administrative Zone 3, Akobo is bordered on the south and west by Sudan, on the northwest by the Alwero River which separates it from Jikawo, and on the southwest by the Administrative Zone 2. Towns in Akobo include Tergol.</obo:IAO_0000115>
        <oboInOwl:hasOBONamespace>GAZ</oboInOwl:hasOBONamespace>
        <oboInOwl:id>GAZ:00123573</oboInOwl:id>
        <rdfs:label>Akobo Woreda</rdfs:label>
    </owl:NamedIndividual>
    


    <!-- http://purl.obolibrary.org/obo/GAZ_00123574 -->

    <owl:NamedIndividual rdf:about="http://purl.obolibrary.org/obo/GAZ_00123574">
        <obo:RO_0001025 rdf:resource="http://purl.obolibrary.org/obo/GAZ_00031109"/>
        <obo:IAO_0000115>One of the eight woredas in the Gambela Region of Ethiopia. Part of the Administrative Zone 3, Jikawo is bordered on the south by the Administrative Zone 2, on the west by the Alwero River which separates it from Akobo, on the north by the Jikawo River which separates it from Sudan, and on the east by the Administrative Zone 1; the Baro River defines Jikawa&apos;s boundary with Sudan and part of the boundary with the Oromia Region. Towns in Jicawo include Telut.</obo:IAO_0000115>
        <oboInOwl:hasOBONamespace>GAZ</oboInOwl:hasOBONamespace>
        <oboInOwl:id>GAZ:00123574</oboInOwl:id>
        <rdfs:label>Jikawo Woreda</rdfs:label>
    </owl:NamedIndividual>
    


    <!-- http://purl.obolibrary.org/obo/GAZ_00123575 -->

    <owl:NamedIndividual rdf:about="http://purl.obolibrary.org/obo/GAZ_00123575">
        <obo:RO_0001025 rdf:resource="http://purl.obolibrary.org/obo/GAZ_00031110"/>
        <obo:IAO_0000115>One of eight woredas in the Gambela Region of Ethiopia. Gambela is the only worera of the Administrative Zone 4 and is considered a Special woreda. Godere is bordered on the south and east by the Southern Nations, Nationalities and Peoples Region, on the west by the Administrative Zone 2 of Gambela, and on the north by the Oromia Region. The only town in Godere is Meti.</obo:IAO_0000115>
        <oboInOwl:hasOBONamespace>GAZ</oboInOwl:hasOBONamespace>
        <oboInOwl:id>GAZ:00123575</oboInOwl:id>
        <rdfs:label>Godere Special Woreda</rdfs:label>
    </owl:NamedIndividual>
    


    <!-- http://purl.obolibrary.org/obo/GAZ_00123576 -->

    <owl:NamedIndividual rdf:about="http://purl.obolibrary.org/obo/GAZ_00123576">
        <obo:RO_0001025 rdf:resource="http://purl.obolibrary.org/obo/GAZ_00031092"/>
        <obo:IAO_0000115>One of the woredas in the chartered city of Dire Dawa in Ethiopia. Towns in Gurgura include Melka Jebdu.</obo:IAO_0000115>
        <oboInOwl:hasOBONamespace>GAZ</oboInOwl:hasOBONamespace>
        <oboInOwl:id>GAZ:00123576</oboInOwl:id>
        <rdfs:label>Gurgura Woreda</rdfs:label>
    </owl:NamedIndividual>
    


    <!-- http://purl.obolibrary.org/obo/GAZ_00123577 -->

    <owl:NamedIndividual rdf:about="http://purl.obolibrary.org/obo/GAZ_00123577">
        <obo:RO_0001025 rdf:resource="http://purl.obolibrary.org/obo/GAZ_00031127"/>
        <obo:IAO_0000115>One of the 47 woredas in the Somali Region of Ethiopia. Part of the Afder Zone, Dolobay is bordered on the south by Somalia, on the west by the Ganale Dorya River which separates it from the Liben Zone, on the northwest by Cherti, on the north by Afder, and on the east by Bare. The major town in Dolobay is Weldiya.</obo:IAO_0000115>
        <oboInOwl:hasOBONamespace>GAZ</oboInOwl:hasOBONamespace>
        <oboInOwl:id>GAZ:00123577</oboInOwl:id>
        <rdfs:label>Dolobay Woreda</rdfs:label>
    </owl:NamedIndividual>
    


    <!-- http://purl.obolibrary.org/obo/GAZ_00123578 -->

    <owl:NamedIndividual rdf:about="http://purl.obolibrary.org/obo/GAZ_00123578">
        <obo:RO_0001025 rdf:resource="http://purl.obolibrary.org/obo/GAZ_00031127"/>
        <obo:IAO_0000115>One of the 47 woredas in the Somali Region of Ethiopia. Part of the Afder Zone, Bare is bordered on the south by Somalia, on the southwest by Dolobay, on the northwest by Afder, on the north by Mirab Imi, and on the east by Shebelle River which separates it from the Gode Zone. The major town in Bare is Bare.</obo:IAO_0000115>
        <oboInOwl:hasOBONamespace>GAZ</oboInOwl:hasOBONamespace>
        <oboInOwl:id>GAZ:00123578</oboInOwl:id>
        <rdfs:label>Bare Woreda</rdfs:label>
    </owl:NamedIndividual>
    


    <!-- http://purl.obolibrary.org/obo/GAZ_00123579 -->

    <owl:NamedIndividual rdf:about="http://purl.obolibrary.org/obo/GAZ_00123579">
        <obo:RO_0001025 rdf:resource="http://purl.obolibrary.org/obo/GAZ_00031127"/>
        <obo:IAO_0000115>One of the 47 woredas in the Somali Region of Ethiopia. It is named for the historically significant village, Imi. Part of the Afder Zone, Mirab Imi is bordered on the south by Bare, on the southwest by Afder, on west by Elekere, and on the north by the Shebelle River which separates it from the Gode Zone. The major town in Mierab Emi is Gudelcha.</obo:IAO_0000115>
        <oboInOwl:hasOBONamespace>GAZ</oboInOwl:hasOBONamespace>
        <oboInOwl:id>GAZ:00123579</oboInOwl:id>
        <rdfs:label>Mirab Imi Woreda</rdfs:label>
    </owl:NamedIndividual>
    


    <!-- http://purl.obolibrary.org/obo/GAZ_00123580 -->

    <owl:NamedIndividual rdf:about="http://purl.obolibrary.org/obo/GAZ_00123580">
        <obo:RO_0001025 rdf:resource="http://purl.obolibrary.org/obo/GAZ_00031127"/>
        <obo:IAO_0000115>One of the 47 woredas in the Somali Region of Ethiopia. Part of the Afder Zone, Guradamole is bounded on the southwest by the Ganale Dorya River which separates it from the Liben Zone, on the west and north by the Oromia Region, on the east by Elekere, and on the southeast by Cherti. Information is not available on the towns and cities of this woreda.</obo:IAO_0000115>
        <oboInOwl:hasOBONamespace>GAZ</oboInOwl:hasOBONamespace>
        <oboInOwl:id>GAZ:00123580</oboInOwl:id>
        <rdfs:label>Guradamole Woreda</rdfs:label>
    </owl:NamedIndividual>
    


    <!-- http://purl.obolibrary.org/obo/GAZ_00123581 -->

    <owl:NamedIndividual rdf:about="http://purl.obolibrary.org/obo/GAZ_00123581">
        <obo:RO_0001025 rdf:resource="http://purl.obolibrary.org/obo/GAZ_00031127"/>
        <obo:IAO_0000115>One of the 47 woredas in the Somali Region of Ethiopia. Part of the Afder Zone, Elekere is bordered on the south by Afder, on the southwest by Cherti, on the northwest by the Oromia Region, on the northeast by the Shebelle River which separates it from the Gode Zone, and on the east by Mirab Imi. The major town in Elekere is Kere.</obo:IAO_0000115>
        <oboInOwl:hasOBONamespace>GAZ</oboInOwl:hasOBONamespace>
        <oboInOwl:id>GAZ:00123581</oboInOwl:id>
        <rdfs:label>Elekere Woreda</rdfs:label>
    </owl:NamedIndividual>
    


    <!-- http://purl.obolibrary.org/obo/GAZ_00123582 -->

    <owl:NamedIndividual rdf:about="http://purl.obolibrary.org/obo/GAZ_00123582">
        <obo:RO_0001025 rdf:resource="http://purl.obolibrary.org/obo/GAZ_00031127"/>
        <obo:IAO_0000115>One of the 47 woredas in the Somali Region of Ethiopia. Part of the Afder Zone, Afder is bordered on the south by Dolobay, on the west by Cherti, on the north by Elekere, on the northwest by Mirab Imi, and on the east by Bare. Towns in Afder include Guda Asbo and Hargele.</obo:IAO_0000115>
        <oboInOwl:hasOBONamespace>GAZ</oboInOwl:hasOBONamespace>
        <oboInOwl:id>GAZ:00123582</oboInOwl:id>
        <rdfs:label>Afder Woreda</rdfs:label>
    </owl:NamedIndividual>
    


    <!-- http://purl.obolibrary.org/obo/GAZ_00123583 -->

    <owl:NamedIndividual rdf:about="http://purl.obolibrary.org/obo/GAZ_00123583">
        <obo:RO_0001025 rdf:resource="http://purl.obolibrary.org/obo/GAZ_00031127"/>
        <obo:IAO_0000115>One of the 47 woredas in the Somali Region of Ethiopia, named after its major town, Cherti. Part of the Afder Zone, Cherti is bordered on the south by the Ganale Dorya River which separates it from the Liben Zone, on the west by Guradamole, on the north by Elekere, on the east by Afder, and on the southeast by Dolobay.</obo:IAO_0000115>
        <oboInOwl:hasOBONamespace>GAZ</oboInOwl:hasOBONamespace>
        <oboInOwl:id>GAZ:00123583</oboInOwl:id>
        <rdfs:label>Cherti Woreda</rdfs:label>
    </owl:NamedIndividual>
    


    <!-- http://purl.obolibrary.org/obo/GAZ_00123584 -->

    <owl:NamedIndividual rdf:about="http://purl.obolibrary.org/obo/GAZ_00123584">
        <obo:RO_0001025 rdf:resource="http://purl.obolibrary.org/obo/GAZ_00031129"/>
        <obo:IAO_0000115>One of the 47 woredas in the Somali Region of Ethiopia. Part of the Degehabur Zone, Degehamedo is bordered on the south and southwest by the Fiq Zone, on the northwest by the Oromia Region, on the northeast by the Jijiga Zone, and on the east by Degehabur. The major town in Degehamedo is Degehamedo.</obo:IAO_0000115>
        <oboInOwl:hasOBONamespace>GAZ</oboInOwl:hasOBONamespace>
        <oboInOwl:id>GAZ:00123584</oboInOwl:id>
        <rdfs:label>Degehamedo Woreda</rdfs:label>
    </owl:NamedIndividual>
    


    <!-- http://purl.obolibrary.org/obo/GAZ_00123585 -->

    <owl:NamedIndividual rdf:about="http://purl.obolibrary.org/obo/GAZ_00123585">
        <obo:RO_0001025 rdf:resource="http://purl.obolibrary.org/obo/GAZ_00031129"/>
        <obo:IAO_0000115>One of the 47 woredas in the Somali Region of Ethiopia. Part of the Degehabur Zone, Aware is bordered on the south by the Korahe Zone, on the west by Degehabur, on the north by the Jijiga Zone, and on the east by Misraq Gashamo.</obo:IAO_0000115>
        <oboInOwl:hasOBONamespace>GAZ</oboInOwl:hasOBONamespace>
        <oboInOwl:id>GAZ:00123585</oboInOwl:id>
        <rdfs:label>Aware Woreda Woreda</rdfs:label>
    </owl:NamedIndividual>
    


    <!-- http://purl.obolibrary.org/obo/GAZ_00123586 -->

    <owl:NamedIndividual rdf:about="http://purl.obolibrary.org/obo/GAZ_00123586">
        <obo:RO_0001025 rdf:resource="http://purl.obolibrary.org/obo/GAZ_00031129"/>
        <obo:IAO_0000115>One of the 47 woredas in the Somali Region of Ethiopia. Part of the Degehabur Zone.</obo:IAO_0000115>
        <oboInOwl:hasOBONamespace>GAZ</oboInOwl:hasOBONamespace>
        <oboInOwl:id>GAZ:00123586</oboInOwl:id>
        <rdfs:label>Gunogado Woreda</rdfs:label>
    </owl:NamedIndividual>
    


    <!-- http://purl.obolibrary.org/obo/GAZ_00123587 -->

    <owl:NamedIndividual rdf:about="http://purl.obolibrary.org/obo/GAZ_00123587">
        <obo:RO_0001025 rdf:resource="http://purl.obolibrary.org/obo/GAZ_00031129"/>
        <obo:IAO_0000115>One of the 47 woredas in the Somali Region of Ethiopia. Part of the Degehabur Zone, Degehabur is bordered on the south by the Gode Zone, on the southwest by the Fiq Zone, on the northwest by Degehamedo, on the north by the Jijiga Zone, on the east by Aware, and on the southeast by the Korahe Zone. The administrative center of this woreda is Degehabur.</obo:IAO_0000115>
        <oboInOwl:hasOBONamespace>GAZ</oboInOwl:hasOBONamespace>
        <oboInOwl:id>GAZ:00123587</oboInOwl:id>
        <rdfs:label>Degehabur Woreda</rdfs:label>
    </owl:NamedIndividual>
    


    <!-- http://purl.obolibrary.org/obo/GAZ_00123588 -->

    <owl:NamedIndividual rdf:about="http://purl.obolibrary.org/obo/GAZ_00123588">
        <obo:RO_0001025 rdf:resource="http://purl.obolibrary.org/obo/GAZ_00031129"/>
        <obo:IAO_0000115>One of the 47 woredas in the Somali Region of Ethiopia. Part of the Degehabur Zone, Misraq Gashamo is bordered on the south by the Werder Zone, on the west by Aware, and on the north and east by Somalia. Towns in Misraq Gashamo include Gashamo and Gowelele.</obo:IAO_0000115>
        <oboInOwl:hasOBONamespace>GAZ</oboInOwl:hasOBONamespace>
        <oboInOwl:id>GAZ:00123588</oboInOwl:id>
        <rdfs:label>Misraq Gashamo Woreda</rdfs:label>
    </owl:NamedIndividual>
    


    <!-- http://purl.obolibrary.org/obo/GAZ_00123589 -->

    <owl:NamedIndividual rdf:about="http://purl.obolibrary.org/obo/GAZ_00123589">
        <obo:RO_0001025 rdf:resource="http://purl.obolibrary.org/obo/GAZ_00031115"/>
        <obo:IAO_0000115>One of the 47 woredas in the Somali Region of Ethiopia, named after its major town, Gerbo. Part of the Fiq Zone, Gerbo is bounded on the southwest by Segeg, and on the north and east by the Degehabur Zone.</obo:IAO_0000115>
        <oboInOwl:hasOBONamespace>GAZ</oboInOwl:hasOBONamespace>
        <oboInOwl:id>GAZ:00123589</oboInOwl:id>
        <rdfs:label>Gerbo Woreda</rdfs:label>
    </owl:NamedIndividual>
    


    <!-- http://purl.obolibrary.org/obo/GAZ_00123590 -->

    <owl:NamedIndividual rdf:about="http://purl.obolibrary.org/obo/GAZ_00123590">
        <obo:RO_0001025 rdf:resource="http://purl.obolibrary.org/obo/GAZ_00031115"/>
        <obo:IAO_0000115>One of the 47 woredas in the Somali Region of Ethiopia, named after its major town, Segeg. Part of the Fiq Zone, Segeg is bordered on the south by Dihun, on the northwest by Hamero, and on the northeast by Gerbo.</obo:IAO_0000115>
        <oboInOwl:hasOBONamespace>GAZ</oboInOwl:hasOBONamespace>
        <oboInOwl:id>GAZ:00123590</oboInOwl:id>
        <rdfs:label>Segeg Woreda</rdfs:label>
    </owl:NamedIndividual>
    


    <!-- http://purl.obolibrary.org/obo/GAZ_00123591 -->

    <owl:NamedIndividual rdf:about="http://purl.obolibrary.org/obo/GAZ_00123591">
        <obo:RO_0001025 rdf:resource="http://purl.obolibrary.org/obo/GAZ_00031115"/>
        <obo:IAO_0000115>One of the 47 woredas in the Somali Region of Ethiopia. Part of the Fiq Zone, Dihun is bordered on the south by the Gode Zone, on the west by the Shebelle River which separates it from the Oromia Region, on the northwest by Hamero, on the northeast by Segeg, and on the east by the Degehabur Zone. The major town in Dihun is Geresley.</obo:IAO_0000115>
        <oboInOwl:hasOBONamespace>GAZ</oboInOwl:hasOBONamespace>
        <oboInOwl:id>GAZ:00123591</oboInOwl:id>
        <rdfs:label>Dihun Woreda</rdfs:label>
    </owl:NamedIndividual>
    


    <!-- http://purl.obolibrary.org/obo/GAZ_00123592 -->

    <owl:NamedIndividual rdf:about="http://purl.obolibrary.org/obo/GAZ_00123592">
        <obo:RO_0001025 rdf:resource="http://purl.obolibrary.org/obo/GAZ_00031115"/>
        <obo:IAO_0000115>One of the 47 woredas in the Somali Region of Ethiopia, named after its major town, Hamero. Part of the Fiq Zone, Hamero is bordered on the south by Dihun, on the west by the Erer and Shebelle Rivers which separate it from the Oromia Region, on the north by Fiq, on the east by the Degehabur Zone, and on the southeast by Segeg.</obo:IAO_0000115>
        <oboInOwl:hasOBONamespace>GAZ</oboInOwl:hasOBONamespace>
        <oboInOwl:id>GAZ:00123592</oboInOwl:id>
        <rdfs:label>Hamero Woreda</rdfs:label>
    </owl:NamedIndividual>
    


    <!-- http://purl.obolibrary.org/obo/GAZ_00123593 -->

    <owl:NamedIndividual rdf:about="http://purl.obolibrary.org/obo/GAZ_00123593">
        <obo:RO_0001025 rdf:resource="http://purl.obolibrary.org/obo/GAZ_00031115"/>
        <obo:IAO_0000115>One of the 47 woredas in the Somali Region of Ethiopia, named after its major town, Fiq. Part of the Fiq Zone, Fiq is bordered on the south by Hamero, on the west and north by the Oromia Region, and on the east by the Degehabur Zone; the woreda&apos;s western boundary is defined by the Erer River.</obo:IAO_0000115>
        <oboInOwl:hasOBONamespace>GAZ</oboInOwl:hasOBONamespace>
        <oboInOwl:id>GAZ:00123593</oboInOwl:id>
        <rdfs:label>Fiq Woreda</rdfs:label>
    </owl:NamedIndividual>
    


    <!-- http://purl.obolibrary.org/obo/GAZ_00123594 -->

    <owl:NamedIndividual rdf:about="http://purl.obolibrary.org/obo/GAZ_00123594">
        <obo:RO_0001025 rdf:resource="http://purl.obolibrary.org/obo/GAZ_00031133"/>
        <obo:IAO_0000115>One of the 47 woredas in the Somali Region of Ethiopia, named after its major town, Danan. Part of the Gode Zone, Danan is bordered on the south by the Shebelle River which separates it from the Afder Zone, on the west by Gode, on the north by the Degehabur Zone, on the east by the Korahe Zone, and on the southeast by Kelafo.</obo:IAO_0000115>
        <oboInOwl:hasOBONamespace>GAZ</oboInOwl:hasOBONamespace>
        <oboInOwl:id>GAZ:00123594</oboInOwl:id>
        <rdfs:label>Danan Woreda</rdfs:label>
    </owl:NamedIndividual>
    


    <!-- http://purl.obolibrary.org/obo/GAZ_00123595 -->

    <owl:NamedIndividual rdf:about="http://purl.obolibrary.org/obo/GAZ_00123595">
        <obo:RO_0001025 rdf:resource="http://purl.obolibrary.org/obo/GAZ_00031133"/>
        <obo:IAO_0000115>One of the 47 woredas in the Somali Region of Ethiopia, named after its major town, Ferfer. Part of the Gode Zone, Ferfer is bordered on the on the west by Mustahil, on the northwest by the Korahe Zone, on the north by the Werder Zone, and on the east and south by Somalia.</obo:IAO_0000115>
        <oboInOwl:hasOBONamespace>GAZ</oboInOwl:hasOBONamespace>
        <oboInOwl:id>GAZ:00123595</oboInOwl:id>
        <rdfs:label>Ferfer Woreda</rdfs:label>
    </owl:NamedIndividual>
    


    <!-- http://purl.obolibrary.org/obo/GAZ_00123596 -->

    <owl:NamedIndividual rdf:about="http://purl.obolibrary.org/obo/GAZ_00123596">
        <obo:RO_0001025 rdf:resource="http://purl.obolibrary.org/obo/GAZ_00031133"/>
        <obo:IAO_0000115>One of the 47 woredas in the Somali Region of Ethiopia. Part of the Gode Zone, Mustahil is bordered on the south by the Shebelle River which separates it from the Afder Zone, on the west by Kelafo, on the north by the Korahe Zone, and on the east by Ferfer. The major town in this woreda is Mustahil.</obo:IAO_0000115>
        <oboInOwl:hasOBONamespace>GAZ</oboInOwl:hasOBONamespace>
        <oboInOwl:id>GAZ:00123596</oboInOwl:id>
        <rdfs:label>Mustahil Woreda</rdfs:label>
    </owl:NamedIndividual>
    


    <!-- http://purl.obolibrary.org/obo/GAZ_00123597 -->

    <owl:NamedIndividual rdf:about="http://purl.obolibrary.org/obo/GAZ_00123597">
        <obo:RO_0001025 rdf:resource="http://purl.obolibrary.org/obo/GAZ_00031133"/>
        <obo:IAO_0000115>One of the 47 woredas in the Somali Region of Ethiopia. Part of the Gode Zone, Kelafo is bordered on the south by the Shebelle River which separates it from the Afder Zone, on the west by Danan, on the north by the Korahe Zone, and on the east by Mustahil. The major town in Kelafo is Kelafo.</obo:IAO_0000115>
        <oboInOwl:hasOBONamespace>GAZ</oboInOwl:hasOBONamespace>
        <oboInOwl:id>GAZ:00123597</oboInOwl:id>
        <rdfs:label>Kelafo Woreda</rdfs:label>
    </owl:NamedIndividual>
    


    <!-- http://purl.obolibrary.org/obo/GAZ_00123598 -->

    <owl:NamedIndividual rdf:about="http://purl.obolibrary.org/obo/GAZ_00123598">
        <obo:RO_0001025 rdf:resource="http://purl.obolibrary.org/obo/GAZ_00031133"/>
        <obo:IAO_0000115>One of the 47 woredas in the Somali Region of Ethiopia, named after its major town, Gode. Part of the Gode Zone, available maps disagree on its exact location. According to the OCHA map for the Somali Region, Gode is bordered on the south and west by the Afder Zone, on the west by the Oromia Region, on the north by the Fiq Zone, and on the east by Danan; the Shebelle River forms the southern and eastern boundaries of the woreda. However, the map of the Oromia Region published by Disaster Prevention and Disaster Agency (DPPA) shows Gode further to the east, bordered on the south by the Shebelle River which separates it from Adadle, on the west by where the OCHA map places Gode (but the DPPA shows is divided into Misraq Imi and Gudis), on the north by Danan, on the northeast by the Korahe Zone, and on the southeast by Kelafo.</obo:IAO_0000115>
        <oboInOwl:hasOBONamespace>GAZ</oboInOwl:hasOBONamespace>
        <oboInOwl:id>GAZ:00123598</oboInOwl:id>
        <rdfs:label>Gode Woreda</rdfs:label>
    </owl:NamedIndividual>
    


    <!-- http://purl.obolibrary.org/obo/GAZ_00123599 -->

    <owl:NamedIndividual rdf:about="http://purl.obolibrary.org/obo/GAZ_00123599">
        <obo:RO_0001025 rdf:resource="http://purl.obolibrary.org/obo/GAZ_00031131"/>
        <obo:IAO_0000115>One of the 47 woredas in the Somali Region of Ethiopia. It is named after one of the 12 major tribes of the Oromo people, the Babille Oromo.</obo:IAO_0000115>
        <oboInOwl:hasOBONamespace>GAZ</oboInOwl:hasOBONamespace>
        <oboInOwl:id>GAZ:00123599</oboInOwl:id>
        <rdfs:label>Babille Woreda</rdfs:label>
    </owl:NamedIndividual>
    


    <!-- http://purl.obolibrary.org/obo/GAZ_00123600 -->

    <owl:NamedIndividual rdf:about="http://purl.obolibrary.org/obo/GAZ_00123600">
        <obo:RO_0001025 rdf:resource="http://purl.obolibrary.org/obo/GAZ_00031131"/>
        <obo:IAO_0000115>One of the 47 woredas in the Somali Region of Ethiopia. Part of the Jijiga Zone, Harshin is bordered on the south by the Degehabur Zone, on the west by Kebri Beyah, and on the east by Somalia. The major town in Harshin is Harshin.</obo:IAO_0000115>
        <oboInOwl:hasOBONamespace>GAZ</oboInOwl:hasOBONamespace>
        <oboInOwl:id>GAZ:00123600</oboInOwl:id>
        <rdfs:label>Harshin Woreda</rdfs:label>
    </owl:NamedIndividual>
    


    <!-- http://purl.obolibrary.org/obo/GAZ_00123601 -->

    <owl:NamedIndividual rdf:about="http://purl.obolibrary.org/obo/GAZ_00123601">
        <obo:RO_0001025 rdf:resource="http://purl.obolibrary.org/obo/GAZ_00031131"/>
        <obo:IAO_0000115>One of the 47 woredas in the Somali Region of Ethiopia. Part of the Jijiga Zone, Kebri Beyah is bordered on the south by the Degehabur Zone, on the west by the Oromia Region, on the northwest by Jijiga, on the north by Awbere, on the northeast by Somalia, and on the southeast by Harshin. Towns in Kebri Beyah include Kebri Beyah and Hart Sheik.</obo:IAO_0000115>
        <oboInOwl:hasOBONamespace>GAZ</oboInOwl:hasOBONamespace>
        <oboInOwl:id>GAZ:00123601</oboInOwl:id>
        <rdfs:label>Kebri Beyah Woreda</rdfs:label>
    </owl:NamedIndividual>
    


    <!-- http://purl.obolibrary.org/obo/GAZ_00123602 -->

    <owl:NamedIndividual rdf:about="http://purl.obolibrary.org/obo/GAZ_00123602">
        <obo:RO_0001025 rdf:resource="http://purl.obolibrary.org/obo/GAZ_00031131"/>
        <obo:IAO_0000115>One of the 47 woredas in the Somali Region of Ethiopia. Part of the Jijiga Zone, Gursum is bordered on the south by Babille, on the west by the Oromia Region, and on the north and east by Jijiga.</obo:IAO_0000115>
        <oboInOwl:hasOBONamespace>GAZ</oboInOwl:hasOBONamespace>
        <oboInOwl:id>GAZ:00123602</oboInOwl:id>
        <rdfs:label>Gursum Woreda</rdfs:label>
    </owl:NamedIndividual>
    


    <!-- http://purl.obolibrary.org/obo/GAZ_00123603 -->

    <owl:NamedIndividual rdf:about="http://purl.obolibrary.org/obo/GAZ_00123603">
        <obo:RO_0001025 rdf:resource="http://purl.obolibrary.org/obo/GAZ_00031131"/>
        <obo:IAO_0000115>One of the 47 woredas in the Somali Region of Ethiopia. Part of the Jijiga Zone, Jijiga is bordered on the south by Babille, on the southwest by Gursum, on the west by the Oromia Region, on the north by the Shinile Zone, on the northeast by Awbere and on the southeast by the Degehabur Zone. Towns and cities in Jijiga include Jijiga and Chinhahsan.</obo:IAO_0000115>
        <oboInOwl:hasOBONamespace>GAZ</oboInOwl:hasOBONamespace>
        <oboInOwl:id>GAZ:00123603</oboInOwl:id>
        <rdfs:label>Jijiga Woreda</rdfs:label>
    </owl:NamedIndividual>
    


    <!-- http://purl.obolibrary.org/obo/GAZ_00123604 -->

    <owl:NamedIndividual rdf:about="http://purl.obolibrary.org/obo/GAZ_00123604">
        <obo:RO_0001025 rdf:resource="http://purl.obolibrary.org/obo/GAZ_00031131"/>
        <obo:IAO_0000115>Awbere is one of the 47 woredas in the Somali Region of Ethiopia. Part of the Jijiga Zone, Awbere is bordered on the southwest by Jijiga, on the west and north by the Shinile Zone, on the east by Somalia, and on the southeast by Kebri Beyah. Towns in Awbere include Awbere and Derwonaji.</obo:IAO_0000115>
        <oboInOwl:hasOBONamespace>GAZ</oboInOwl:hasOBONamespace>
        <oboInOwl:id>GAZ:00123604</oboInOwl:id>
        <rdfs:label>Awbere Woreda</rdfs:label>
    </owl:NamedIndividual>
    


    <!-- http://purl.obolibrary.org/obo/GAZ_00123605 -->

    <owl:NamedIndividual rdf:about="http://purl.obolibrary.org/obo/GAZ_00123605">
        <obo:RO_0001025 rdf:resource="http://purl.obolibrary.org/obo/GAZ_00031130"/>
        <obo:IAO_0000115>One of the 47 woredas in the Somali Region of Ethiopia. Part of the Korahe Zone, Kebri Dar is bordered on the south by Debeweyin, on the west by the Gode Zone, on the northwest by the Degehabur Zone, on the north by Shekosh, on the east by the Werder Zone, and on the southeast by Shilavo. The major town in Kebri Dahar is Kebri Dahar.</obo:IAO_0000115>
        <oboInOwl:hasOBONamespace>GAZ</oboInOwl:hasOBONamespace>
        <oboInOwl:id>GAZ:00123605</oboInOwl:id>
        <rdfs:label>Kebri Dahar Woreda</rdfs:label>
    </owl:NamedIndividual>
    


    <!-- http://purl.obolibrary.org/obo/GAZ_00123606 -->

    <owl:NamedIndividual rdf:about="http://purl.obolibrary.org/obo/GAZ_00123606">
        <obo:RO_0001025 rdf:resource="http://purl.obolibrary.org/obo/GAZ_00031130"/>
        <obo:IAO_0000115>One of the 47 woredas in the Somali Region of Ethiopia. Part of the Korahe Zone, Debeweyin is bordered on the south and west by the Gode Zone, on the north by Kebri Dahar, and on the east by Shilavo. The major town in Debeweyin is Har Ad.</obo:IAO_0000115>
        <oboInOwl:hasOBONamespace>GAZ</oboInOwl:hasOBONamespace>
        <oboInOwl:id>GAZ:00123606</oboInOwl:id>
        <rdfs:label>Debeweyin Woreda</rdfs:label>
    </owl:NamedIndividual>
    


    <!-- http://purl.obolibrary.org/obo/GAZ_00123607 -->

    <owl:NamedIndividual rdf:about="http://purl.obolibrary.org/obo/GAZ_00123607">
        <obo:RO_0001025 rdf:resource="http://purl.obolibrary.org/obo/GAZ_00031130"/>
        <obo:IAO_0000115>One of the 47 woredas in the Somali Region of Ethiopia. Part of the Korahe Zone, its boundaries shown by official sources vary. On the OCHA map for the Somali Region (copyright 2003), Shilavo is bordered on the south by the Gode Zone, on the southwest by Debeweyin, on the north by Kebri Dahar, and on the east by the Werder Zone.</obo:IAO_0000115>
        <oboInOwl:hasOBONamespace>GAZ</oboInOwl:hasOBONamespace>
        <oboInOwl:id>GAZ:00123607</oboInOwl:id>
        <rdfs:label>Shekosh Woreda</rdfs:label>
    </owl:NamedIndividual>
    


    <!-- http://purl.obolibrary.org/obo/GAZ_00123608 -->

    <owl:NamedIndividual rdf:about="http://purl.obolibrary.org/obo/GAZ_00123608">
        <obo:RO_0001025 rdf:resource="http://purl.obolibrary.org/obo/GAZ_00031130"/>
        <obo:IAO_0000115>One of the 47 woredas in the Somali Region of Ethiopia. Part of the Korahe Zone, Shekosh is bordered on the south by Kebri Dahar, on the north by the Degehabur Zone, and on the east by the Werder Zone. The major town in Shekosh is Shekosh.</obo:IAO_0000115>
        <oboInOwl:hasOBONamespace>GAZ</oboInOwl:hasOBONamespace>
        <oboInOwl:id>GAZ:00123608</oboInOwl:id>
        <rdfs:label>Shilavo Woreda</rdfs:label>
    </owl:NamedIndividual>
    


    <!-- http://purl.obolibrary.org/obo/GAZ_00123609 -->

    <owl:NamedIndividual rdf:about="http://purl.obolibrary.org/obo/GAZ_00123609">
        <obo:RO_0001025 rdf:resource="http://purl.obolibrary.org/obo/GAZ_00031126"/>
        <obo:IAO_0000115>One of the 47 woredas in the Somali Region of Ethiopia. Part of the Liben Zone, Dolo Odo is located in the angle formed by the confluence of the Ganale Dorya with the Dawa River, and bordered to the west by Liben. Towns in Dolo Odo include Bekol May, Dolo and Softu.</obo:IAO_0000115>
        <oboInOwl:hasOBONamespace>GAZ</oboInOwl:hasOBONamespace>
        <oboInOwl:id>GAZ:00123609</oboInOwl:id>
        <rdfs:label>Dolo Odo Woreda</rdfs:label>
    </owl:NamedIndividual>
    


    <!-- http://purl.obolibrary.org/obo/GAZ_00123610 -->

    <owl:NamedIndividual rdf:about="http://purl.obolibrary.org/obo/GAZ_00123610">
        <obo:RO_0001025 rdf:resource="http://purl.obolibrary.org/obo/GAZ_00031126"/>
        <obo:IAO_0000115>One of the 47 woredas in the Somali Region of Ethiopia. Part of the Liben Zone, Liben is bordered on the south by the Dawa River which separates it from Kenya, on the west and north by the Oromia Region, on the north and east by the Ganale Dorya River which separates it from the Afder Zone, and on the east by Dolo Odo. The major town in Liben is Filtu.</obo:IAO_0000115>
        <oboInOwl:hasOBONamespace>GAZ</oboInOwl:hasOBONamespace>
        <oboInOwl:id>GAZ:00123610</oboInOwl:id>
        <rdfs:label>Liben Woreda</rdfs:label>
    </owl:NamedIndividual>
    


    <!-- http://purl.obolibrary.org/obo/GAZ_00123611 -->

    <owl:NamedIndividual rdf:about="http://purl.obolibrary.org/obo/GAZ_00123611">
        <obo:RO_0001025 rdf:resource="http://purl.obolibrary.org/obo/GAZ_00031126"/>
        <obo:IAO_0000115>One of the 47 woredas in the Somali Region of Ethiopia. The population estimates of the Central Statistical Agency (CSA) include Moyale as part of the Liben Zone; however, this woreda is not shown on the OCHA map for the Somali Region. Towns in this woreda include Chelago.</obo:IAO_0000115>
        <oboInOwl:hasOBONamespace>GAZ</oboInOwl:hasOBONamespace>
        <oboInOwl:id>GAZ:00123611</oboInOwl:id>
        <rdfs:label>Moyale Woreda</rdfs:label>
    </owl:NamedIndividual>
    


    <!-- http://purl.obolibrary.org/obo/GAZ_00123612 -->

    <owl:NamedIndividual rdf:about="http://purl.obolibrary.org/obo/GAZ_00123612">
        <obo:RO_0001025 rdf:resource="http://purl.obolibrary.org/obo/GAZ_00031128"/>
        <obo:IAO_0000115>One of the 47 woredas in the Somali Region of Ethiopia. Part of the Shinile Zone, Dembel is bordered on the southwest by the Oromia Region, on the west by Dire Dawa, on the northwest by Shinile, on the northeast by Ayesha, and on the east and south by the Jijiga Zone. Towns in Dembel include Arebi, Biyo Behay, Dembel, Dure, Harmukale, and Smekeb.</obo:IAO_0000115>
        <oboInOwl:hasOBONamespace>GAZ</oboInOwl:hasOBONamespace>
        <oboInOwl:id>GAZ:00123612</oboInOwl:id>
        <rdfs:label>Dembela Woreda</rdfs:label>
    </owl:NamedIndividual>
    


    <!-- http://purl.obolibrary.org/obo/GAZ_00123613 -->

    <owl:NamedIndividual rdf:about="http://purl.obolibrary.org/obo/GAZ_00123613">
        <obo:RO_0001025 rdf:resource="http://purl.obolibrary.org/obo/GAZ_00031128"/>
        <obo:IAO_0000115>One of the 47 woredas in the Somali Region of Ethiopia. Part of the Shinile Zone, Shinile is bordered on the south by Dire Dawa, on the west by Erer, on the north and east by Ayesha, and on the southeast by Dembel. Towns in Shinile include Adigale, Harewa, Milo, and Shinile.</obo:IAO_0000115>
        <oboInOwl:hasOBONamespace>GAZ</oboInOwl:hasOBONamespace>
        <oboInOwl:id>GAZ:00123613</oboInOwl:id>
        <rdfs:label>Shinilea Woreda</rdfs:label>
    </owl:NamedIndividual>
    


    <!-- http://purl.obolibrary.org/obo/GAZ_00123614 -->

    <owl:NamedIndividual rdf:about="http://purl.obolibrary.org/obo/GAZ_00123614">
        <obo:RO_0001025 rdf:resource="http://purl.obolibrary.org/obo/GAZ_00031128"/>
        <obo:IAO_0000115>One of the 47 woredas in the Somali Region of Ethiopia. The population estimates of the Central Statistical Agency (CSA) include Mieso as part of the Shinile Zone; however, this woreda is not shown on the OCHA map for the Somali Region.</obo:IAO_0000115>
        <oboInOwl:hasOBONamespace>GAZ</oboInOwl:hasOBONamespace>
        <oboInOwl:id>GAZ:00123614</oboInOwl:id>
        <rdfs:label>Miesoa Woreda</rdfs:label>
    </owl:NamedIndividual>
    


    <!-- http://purl.obolibrary.org/obo/GAZ_00123615 -->

    <owl:NamedIndividual rdf:about="http://purl.obolibrary.org/obo/GAZ_00123615">
        <obo:RO_0001025 rdf:resource="http://purl.obolibrary.org/obo/GAZ_00031128"/>
        <obo:IAO_0000115>One of the 47 woredas in the Somali Region of Ethiopia. The northernmost woreda of the Shinile Zone, Ayesha is bordered on the south by Dembel, on the southwest by Shinile, on the west by Erer, on the north by Djibouti, on the east by Somalia, and on the southeast by the Jijiga Zone. Towns in Ayesha include Ayesha, Dewele, Laserat and Mermedebis.</obo:IAO_0000115>
        <oboInOwl:hasOBONamespace>GAZ</oboInOwl:hasOBONamespace>
        <oboInOwl:id>GAZ:00123615</oboInOwl:id>
        <rdfs:label>Ayesha Woreda</rdfs:label>
    </owl:NamedIndividual>
    


    <!-- http://purl.obolibrary.org/obo/GAZ_00123616 -->

    <owl:NamedIndividual rdf:about="http://purl.obolibrary.org/obo/GAZ_00123616">
        <obo:RO_0001025 rdf:resource="http://purl.obolibrary.org/obo/GAZ_00031128"/>
        <obo:IAO_0000115>One of the 47 woredas in the Somali Region of Ethiopia. Part of the Shinile Zone, available maps disagree on its exact location: according to the OCHA map for the Somali Region, Erer is bordered on the south by the Oromia Region, on the southwest by Afdem, on the west by the Afar Region, on the north by Djibouti, on the northeast by Ayesha, on the east by Shinile and the southeast by the territory of Dire Dawa; however, the map of the Oromia Region published by Disaster Prevention and Disaster Agency shows that the western part is separated into its own woreda called Afdem, and the woreda the OCHA map identifies as Afdem should be named Mieso.</obo:IAO_0000115>
        <oboInOwl:hasOBONamespace>GAZ</oboInOwl:hasOBONamespace>
        <oboInOwl:id>GAZ:00123616</oboInOwl:id>
        <rdfs:label>Erera Woreda</rdfs:label>
    </owl:NamedIndividual>
    


    <!-- http://purl.obolibrary.org/obo/GAZ_00123617 -->

    <owl:NamedIndividual rdf:about="http://purl.obolibrary.org/obo/GAZ_00123617">
        <obo:RO_0001025 rdf:resource="http://purl.obolibrary.org/obo/GAZ_00031128"/>
        <obo:IAO_0000115>One of the 47 woredas in the Somali Region of Ethiopia. Part of the Shinile Zone, available maps disagree on its exact location: according to the OCHA map for the Somali Region, Afdem is located in the westernmost part of the Zone, and is bordered on the south by the Oromia Region, on the west by the Afar Region, and on the north and east by Erer; however, the map of the Oromia Region published by Disaster Prevention and Disaster Agency shows Afdem is the woreda immediately to the east of the woreda with these boundaries (which it calls Mieso), and shows that it is bordered on the south by the Oromia Region, on the southwest by Mieso, and on the northwest and north by the Afar Region and on the east by Erer.</obo:IAO_0000115>
        <oboInOwl:hasOBONamespace>GAZ</oboInOwl:hasOBONamespace>
        <oboInOwl:id>GAZ:00123617</oboInOwl:id>
        <rdfs:label>Afdema Woreda</rdfs:label>
    </owl:NamedIndividual>
    


    <!-- http://purl.obolibrary.org/obo/GAZ_00123618 -->

    <owl:NamedIndividual rdf:about="http://purl.obolibrary.org/obo/GAZ_00123618">
        <obo:RO_0001025 rdf:resource="http://purl.obolibrary.org/obo/GAZ_00031132"/>
        <obo:IAO_0000115>One of the 47 woredas in the Somali Region of Ethiopia. Part of the Werder Zone, Boh is located in the easternmost part of the country, at the point of the angle jutting into Somalia. It is bordered on the southwest by Geladin, and on the northwest by Danot. Towns and cities in Boh include Boh and Dimeriad.</obo:IAO_0000115>
        <oboInOwl:hasOBONamespace>GAZ</oboInOwl:hasOBONamespace>
        <oboInOwl:id>GAZ:00123618</oboInOwl:id>
        <rdfs:label>Boh Woreda</rdfs:label>
    </owl:NamedIndividual>
    


    <!-- http://purl.obolibrary.org/obo/GAZ_00123619 -->

    <owl:NamedIndividual rdf:about="http://purl.obolibrary.org/obo/GAZ_00123619">
        <obo:RO_0001025 rdf:resource="http://purl.obolibrary.org/obo/GAZ_00031132"/>
        <obo:IAO_0000115>One of the 47 woredas in the Somali Region of Ethiopia, named after its major town, Danot. Part of the Werder Zone, Danot is bordered on the south by Werder, on the west by the Degehabur Zone, on the north by Somalia, and on the east by Boh.</obo:IAO_0000115>
        <oboInOwl:hasOBONamespace>GAZ</oboInOwl:hasOBONamespace>
        <oboInOwl:id>GAZ:00123619</oboInOwl:id>
        <rdfs:label>Danot Woreda</rdfs:label>
    </owl:NamedIndividual>
    


    <!-- http://purl.obolibrary.org/obo/GAZ_00123620 -->

    <owl:NamedIndividual rdf:about="http://purl.obolibrary.org/obo/GAZ_00123620">
        <obo:RO_0001025 rdf:resource="http://purl.obolibrary.org/obo/GAZ_00031132"/>
        <obo:IAO_0000115>One of the 47 woredas in the Somali Region of Ethiopia, named after its administrative center, Werder. Part of the Werder Zone, its boundaries shown by official sources vary. On the OCHA map for the Somali Region, Werder is bordered on the south by the Gode Zone, on the west by the Korahe Zone, on the north by the Degehabur Zone, on the east by Danot, and on the east by Geladin. However on the map of the Ethiopian Disaster Prevention and Preparedness Agency Werder extends east to the national border with Somalia separating Geladin from the Korahe Zone, which shares its boundary on the entire south and east sides.</obo:IAO_0000115>
        <oboInOwl:hasOBONamespace>GAZ</oboInOwl:hasOBONamespace>
        <oboInOwl:id>GAZ:00123620</oboInOwl:id>
        <rdfs:label>Werder Woreda</rdfs:label>
    </owl:NamedIndividual>
    


    <!-- http://purl.obolibrary.org/obo/GAZ_00123621 -->

    <owl:NamedIndividual rdf:about="http://purl.obolibrary.org/obo/GAZ_00123621">
        <obo:RO_0001025 rdf:resource="http://purl.obolibrary.org/obo/GAZ_00031132"/>
        <obo:IAO_0000115>One of the 47 woredas in the Somali Region of Ethiopia. Part of the Werder Zone, its boundaries shown by official sources vary. On the OCHA map for the Somali Region, Geladin is bordered on the south by the Gode Zone, on the west by Werder, on the northeast by Boh, and on the east by Somalia. However on the map of the Ethiopian Disaster Prevention and Preparedness Agency, Werder extends east to the national border with Somalia separating Geladin from the Gode Zone.</obo:IAO_0000115>
        <oboInOwl:hasOBONamespace>GAZ</oboInOwl:hasOBONamespace>
        <oboInOwl:id>GAZ:00123621</oboInOwl:id>
        <rdfs:label>Geladin Woreda</rdfs:label>
    </owl:NamedIndividual>
    


    <!-- http://purl.obolibrary.org/obo/GAZ_00123622 -->

    <owl:NamedIndividual rdf:about="http://purl.obolibrary.org/obo/GAZ_00123622">
        <obo:RO_0001025 rdf:resource="http://purl.obolibrary.org/obo/GAZ_00031147"/>
        <obo:IAO_0000115>One of the 77 woredas in the Southern Nations, Nationalities and Peoples&apos; Region of Ethiopia. It is named after the Dizi people, whose homeland lies in the northern part of this district; a different ethnic group, the Surma, inhabit the southern part. Part of the Bench Maji Zone, Dizi is bordered on the south by the Kibish River which separates it from Sudan, on the west by Surma, on the north by Meinit, and on the east by the Omo River which separates it from the Debub Omo Zone. Towns in Dizi include Tum and Maji.</obo:IAO_0000115>
        <oboInOwl:hasOBONamespace>GAZ</oboInOwl:hasOBONamespace>
        <oboInOwl:id>GAZ:00123622</oboInOwl:id>
        <rdfs:label>Dizi Woreda</rdfs:label>
    </owl:NamedIndividual>
    


    <!-- http://purl.obolibrary.org/obo/GAZ_00123623 -->

    <owl:NamedIndividual rdf:about="http://purl.obolibrary.org/obo/GAZ_00123623">
        <obo:RO_0001025 rdf:resource="http://purl.obolibrary.org/obo/GAZ_00031147"/>
        <obo:IAO_0000115>One of the 77 woredas in the Southern Nations, Nationalities and Peoples&apos; Region of Ethiopia. Part of the Bench Maji Zone, Meinit is bordered on the south by Dizi, on the west by Sheko, on the north by Bench, on the east by the Keficho Shekicho Zone, and on the southeast by the Omo River which separates it from the Debub Omo Zone. Towns in Meinit include Bachuma, Kela Ketema and Jemu.</obo:IAO_0000115>
        <oboInOwl:hasOBONamespace>GAZ</oboInOwl:hasOBONamespace>
        <oboInOwl:id>GAZ:00123623</oboInOwl:id>
        <rdfs:label>Meinit Woreda</rdfs:label>
    </owl:NamedIndividual>
    


    <!-- http://purl.obolibrary.org/obo/GAZ_00123624 -->

    <owl:NamedIndividual rdf:about="http://purl.obolibrary.org/obo/GAZ_00123624">
        <obo:RO_0001025 rdf:resource="http://purl.obolibrary.org/obo/GAZ_00031147"/>
        <obo:IAO_0000115>One of the 77 woredas in the Southern Nations, Nationalities and Peoples&apos; Region of Ethiopia. Part of the Bench Maji Zone, Sheko is bordered on the south by Dizi, southwest by Surma, on the west by Sudan, on the north by the Gambela Region, on the northeast by Keficho Shekicho Zone, on the east by Bench, and on the southeast by Meinit. Towns in Sheko include Dima, Guraferda and Sheko.</obo:IAO_0000115>
        <oboInOwl:hasOBONamespace>GAZ</oboInOwl:hasOBONamespace>
        <oboInOwl:id>GAZ:00123624</oboInOwl:id>
        <rdfs:label>Sheko Woreda</rdfs:label>
    </owl:NamedIndividual>
    


    <!-- http://purl.obolibrary.org/obo/GAZ_00123625 -->

    <owl:NamedIndividual rdf:about="http://purl.obolibrary.org/obo/GAZ_00123625">
        <obo:RO_0001025 rdf:resource="http://purl.obolibrary.org/obo/GAZ_00031147"/>
        <obo:IAO_0000115>One of the 77 woredas in the Southern Nations, Nationalities and Peoples&apos; Region of Ethiopia. Part of the Bench Maji Zone, Surma is bordered on the south and west by Sudan, on the north by Sheko, and on the east by Dizi. Towns in this woreda include Bambu and Chela. Part of the Omo National Park extends into the southern part of this woreda.</obo:IAO_0000115>
        <oboInOwl:hasOBONamespace>GAZ</oboInOwl:hasOBONamespace>
        <oboInOwl:id>GAZ:00123625</oboInOwl:id>
        <rdfs:label>Surma Woreda</rdfs:label>
    </owl:NamedIndividual>
    


    <!-- http://purl.obolibrary.org/obo/GAZ_00123626 -->

    <owl:NamedIndividual rdf:about="http://purl.obolibrary.org/obo/GAZ_00123626">
        <obo:RO_0001025 rdf:resource="http://purl.obolibrary.org/obo/GAZ_00031147"/>
        <obo:IAO_0000115>One of the 77 woredas in the Southern Nations, Nationalities and Peoples&apos; Region of Ethiopia. Part of the Bench Maji Zone, Bench is bordered on the south and east by Meinit, on the west by Sheko, and on the north by the Keficho Shekicho Zone. Towns in Bench include Aman and Mizan Teferi.</obo:IAO_0000115>
        <oboInOwl:hasOBONamespace>GAZ</oboInOwl:hasOBONamespace>
        <oboInOwl:id>GAZ:00123626</oboInOwl:id>
        <rdfs:label>Bench Woreda</rdfs:label>
    </owl:NamedIndividual>
    


    <!-- http://purl.obolibrary.org/obo/GAZ_00123627 -->

    <owl:NamedIndividual rdf:about="http://purl.obolibrary.org/obo/GAZ_00123627">
        <obo:RO_0001025 rdf:resource="http://purl.obolibrary.org/obo/GAZ_00031136"/>
        <obo:IAO_0000115>One of the 77 woredas in the Southern Nations, Nationalities and Peoples&apos; Region of Ethiopia, named after its major town, Bule. Part of the Gedeo Zone, Bule is bordered on the south by Kochere, on the west by Yirgachefe, on the northwest by Wenago, and on the east by the Oromia Region.</obo:IAO_0000115>
        <oboInOwl:hasOBONamespace>GAZ</oboInOwl:hasOBONamespace>
        <oboInOwl:id>GAZ:00123627</oboInOwl:id>
        <rdfs:label>Bule Woreda</rdfs:label>
    </owl:NamedIndividual>
    


    <!-- http://purl.obolibrary.org/obo/GAZ_00123628 -->

    <owl:NamedIndividual rdf:about="http://purl.obolibrary.org/obo/GAZ_00123628">
        <obo:RO_0001025 rdf:resource="http://purl.obolibrary.org/obo/GAZ_00031136"/>
        <obo:IAO_0000115>One of the 77 woredas in the Southern Nations, Nationalities and Peoples&apos; Region of Ethiopia. Part of the Gedeo Zone, Kochere is bordered on the east, south and west by the Oromia Region, on the north by Yirgachefe, and on the northeast by Bule. Towns in Kochere include Fisehagenet and Chelelektu.</obo:IAO_0000115>
        <oboInOwl:hasOBONamespace>GAZ</oboInOwl:hasOBONamespace>
        <oboInOwl:id>GAZ:00123628</oboInOwl:id>
        <rdfs:label>Kochere Woreda</rdfs:label>
    </owl:NamedIndividual>
    


    <!-- http://purl.obolibrary.org/obo/GAZ_00123629 -->

    <owl:NamedIndividual rdf:about="http://purl.obolibrary.org/obo/GAZ_00123629">
        <obo:RO_0001025 rdf:resource="http://purl.obolibrary.org/obo/GAZ_00031136"/>
        <obo:IAO_0000115>One of the 77 woredas in the Southern Nations, Nationalities and Peoples&apos; Region of Ethiopia. Part of the Gedeo Zone, Yirgachefe is bordered on the south by Kochere, on the west by the Oromia Zone, on the north by Wenago, and on the east by Bule.</obo:IAO_0000115>
        <oboInOwl:hasOBONamespace>GAZ</oboInOwl:hasOBONamespace>
        <oboInOwl:id>GAZ:00123629</oboInOwl:id>
        <rdfs:label>Yirgachefe Woreda</rdfs:label>
    </owl:NamedIndividual>
    


    <!-- http://purl.obolibrary.org/obo/GAZ_00123630 -->

    <owl:NamedIndividual rdf:about="http://purl.obolibrary.org/obo/GAZ_00123630">
        <obo:RO_0001025 rdf:resource="http://purl.obolibrary.org/obo/GAZ_00031136"/>
        <obo:IAO_0000115>One of the 77 woredas in the Southern Nations, Nationalities and Peoples&apos; Region of Ethiopia. Part of the Gedeo Zone, Wenago is bordered on the south by Yirgachefe, on the west by the Oromia Region, on the north by the Sidama Zone, and on the east by Bule. Towns in Wenago include Wenago and Dilla.</obo:IAO_0000115>
        <oboInOwl:hasOBONamespace>GAZ</oboInOwl:hasOBONamespace>
        <oboInOwl:id>GAZ:00123630</oboInOwl:id>
        <rdfs:label>Wenago Woreda</rdfs:label>
    </owl:NamedIndividual>
    


    <!-- http://purl.obolibrary.org/obo/GAZ_00123631 -->

    <owl:NamedIndividual rdf:about="http://purl.obolibrary.org/obo/GAZ_00123631">
        <obo:RO_0001025 rdf:resource="http://purl.obolibrary.org/obo/GAZ_00031146"/>
        <obo:IAO_0000115>One of the 77 woredas in the Southern Nations, Nationalities and Peoples&apos; Region of Ethiopia. Part of the Gurage Zone, Ezhana Wolene is bordered on the south by Gumer, on the west by Cheha, on the north by Goro, on the northeast by Kokir Gedebano Gutazer, and on the east by Meskanena Mareko.</obo:IAO_0000115>
        <oboInOwl:hasOBONamespace>GAZ</oboInOwl:hasOBONamespace>
        <oboInOwl:id>GAZ:00123631</oboInOwl:id>
        <rdfs:label>Ezhana Wolene Woreda</rdfs:label>
    </owl:NamedIndividual>
    


    <!-- http://purl.obolibrary.org/obo/GAZ_00123632 -->

    <owl:NamedIndividual rdf:about="http://purl.obolibrary.org/obo/GAZ_00123632">
        <obo:RO_0001025 rdf:resource="http://purl.obolibrary.org/obo/GAZ_00031146"/>
        <obo:IAO_0000115>One of the 77 woredas in the Southern Nations, Nationalities and Peoples&apos; Region of Ethiopia. Part of the Gurage Zone, Meskanena Mareko is bordered on the south by Silte, on the southwest by Gumer, on the west by Ezhana Wolene, on the northwest by Kokir Gedebano Gutazer, on the north by Sodo, and on the east by the Oromia Region. Towns in Meskanena Mareko include Butajira and Inseno.</obo:IAO_0000115>
        <oboInOwl:hasOBONamespace>GAZ</oboInOwl:hasOBONamespace>
        <oboInOwl:id>GAZ:00123632</oboInOwl:id>
        <rdfs:label>Meskanena Mareko Woreda</rdfs:label>
    </owl:NamedIndividual>
    


    <!-- http://purl.obolibrary.org/obo/GAZ_00123633 -->

    <owl:NamedIndividual rdf:about="http://purl.obolibrary.org/obo/GAZ_00123633">
        <obo:RO_0001025 rdf:resource="http://purl.obolibrary.org/obo/GAZ_00031146"/>
        <obo:IAO_0000115>One of the 77 woredas in the Southern Nations, Nationalities and Peoples&apos; Region of Ethiopia. Part of the Gurage Zone, Sodo is bordered on the south by Meskanena Mareko, and on the west, north and east by the Oromia Region. Towns in Sodo include Bue and Kela.</obo:IAO_0000115>
        <oboInOwl:hasOBONamespace>GAZ</oboInOwl:hasOBONamespace>
        <oboInOwl:id>GAZ:00123633</oboInOwl:id>
        <rdfs:label>Sodo Woreda</rdfs:label>
    </owl:NamedIndividual>
    


    <!-- http://purl.obolibrary.org/obo/GAZ_00123634 -->

    <owl:NamedIndividual rdf:about="http://purl.obolibrary.org/obo/GAZ_00123634">
        <obo:RO_0001025 rdf:resource="http://purl.obolibrary.org/obo/GAZ_00031146"/>
        <obo:IAO_0000115>One of the 77 woredas in the Southern Nations, Nationalities and Peoples&apos; Region of Ethiopia. Part of the Gurage Zone, Goro is bordered on the south by Cheha, on the west and north by the Oromia Region, on the farther east by Kokir Gedebano Gutazer, and on the southeast by Ezhana Wolene.</obo:IAO_0000115>
        <oboInOwl:hasOBONamespace>GAZ</oboInOwl:hasOBONamespace>
        <oboInOwl:id>GAZ:00123634</oboInOwl:id>
        <rdfs:label>Goro Woreda</rdfs:label>
    </owl:NamedIndividual>
    


    <!-- http://purl.obolibrary.org/obo/GAZ_00123635 -->

    <owl:NamedIndividual rdf:about="http://purl.obolibrary.org/obo/GAZ_00123635">
        <obo:RO_0001025 rdf:resource="http://purl.obolibrary.org/obo/GAZ_00031146"/>
        <obo:IAO_0000115>One of the 77 woredas in the Southern Nations, Nationalities and Peoples&apos; Region of Ethiopia. Part of the Gurage Zone, Silte is bordered on the southeast by Lanfro, on the southwest by Dalocha, on the northwest by Gumer, and on the northeast by Meskanena Mareko. Towns in Silte include Alkaso, Worabe and Kibet.</obo:IAO_0000115>
        <oboInOwl:hasOBONamespace>GAZ</oboInOwl:hasOBONamespace>
        <oboInOwl:id>GAZ:00123635</oboInOwl:id>
        <rdfs:label>Silte Woreda</rdfs:label>
    </owl:NamedIndividual>
    


    <!-- http://purl.obolibrary.org/obo/GAZ_00123636 -->

    <owl:NamedIndividual rdf:about="http://purl.obolibrary.org/obo/GAZ_00123636">
        <obo:RO_0001025 rdf:resource="http://purl.obolibrary.org/obo/GAZ_00031146"/>
        <obo:IAO_0000115>One of the 77 woredas in the Southern Nations, Nationalities and Peoples&apos; Region of Ethiopia. Part of the Gurage Zone, Kokir Gedebano Gutazer is bordered on the south by Ezhana Wolene, on the west by Goro, on the north by the Oromia Region, and on the east by Meskanena Mareko.</obo:IAO_0000115>
        <oboInOwl:hasOBONamespace>GAZ</oboInOwl:hasOBONamespace>
        <oboInOwl:id>GAZ:00123636</oboInOwl:id>
        <rdfs:label>Kokir Gedebano Gutazer Woreda</rdfs:label>
    </owl:NamedIndividual>
    


    <!-- http://purl.obolibrary.org/obo/GAZ_00123637 -->

    <owl:NamedIndividual rdf:about="http://purl.obolibrary.org/obo/GAZ_00123637">
        <obo:RO_0001025 rdf:resource="http://purl.obolibrary.org/obo/GAZ_00031146"/>
        <obo:IAO_0000115>One of the 77 woredas in the Southern Nations, Nationalities and Peoples&apos; Region of Ethiopia. Part of the Gurage Zone, Lanfro is bordered on the south by the Kembata Alaba and Tembaro Zone, on the west by Dalocha, on the north by Silte, and on the east by the Oromia Region. The major town in Lanfro is Torra.</obo:IAO_0000115>
        <oboInOwl:hasOBONamespace>GAZ</oboInOwl:hasOBONamespace>
        <oboInOwl:id>GAZ:00123637</oboInOwl:id>
        <rdfs:label>Lanfro Woreda</rdfs:label>
    </owl:NamedIndividual>
    


    <!-- http://purl.obolibrary.org/obo/GAZ_00123638 -->

    <owl:NamedIndividual rdf:about="http://purl.obolibrary.org/obo/GAZ_00123638">
        <obo:RO_0001025 rdf:resource="http://purl.obolibrary.org/obo/GAZ_00031146"/>
        <obo:IAO_0000115>One of the 77 woredas in the Southern Nations, Nationalities and Peoples&apos; Region of Ethiopia. Part of the Gurage Zone, Gumer is bordered on the south by the Hadiya Zone, on the west by Enemorina Eaner, on the northwest by Cheha, on the north by Ezhana Wolene, on the northeast by Meskanena Mareko, and on the east by Silte. Towns in Gumer include Arkit and Kebul.</obo:IAO_0000115>
        <oboInOwl:hasOBONamespace>GAZ</oboInOwl:hasOBONamespace>
        <oboInOwl:id>GAZ:00123638</oboInOwl:id>
        <rdfs:label>Gumer Woreda</rdfs:label>
    </owl:NamedIndividual>
    


    <!-- http://purl.obolibrary.org/obo/GAZ_00123639 -->

    <owl:NamedIndividual rdf:about="http://purl.obolibrary.org/obo/GAZ_00123639">
        <obo:RO_0001025 rdf:resource="http://purl.obolibrary.org/obo/GAZ_00031146"/>
        <obo:IAO_0000115>One of the 77 woredas in the Southern Nations, Nationalities and Peoples&apos; Region of Ethiopia. Part of the Gurage Zone, Cheha is bordered on the south by Enemorina Eaner, on the west by the Oromia Region, on the north by Goro, on the east by Ezhana Wolene, and on the southeast by Gumer. Towns in Cheha include Endibir and Gubre.</obo:IAO_0000115>
        <oboInOwl:hasOBONamespace>GAZ</oboInOwl:hasOBONamespace>
        <oboInOwl:id>GAZ:00123639</oboInOwl:id>
        <rdfs:label>Cheha Woreda</rdfs:label>
    </owl:NamedIndividual>
    


    <!-- http://purl.obolibrary.org/obo/GAZ_00123640 -->

    <owl:NamedIndividual rdf:about="http://purl.obolibrary.org/obo/GAZ_00123640">
        <obo:RO_0001025 rdf:resource="http://purl.obolibrary.org/obo/GAZ_00031146"/>
        <obo:IAO_0000115>One of the 77 woredas in the Southern Nations, Nationalities and Peoples&apos; Region of Ethiopia. Part of the Gurage Zone, Enemorina Eaner is bordered on the south by the Hadiya Zone, on the west by Oromia Region, on the north by Cheha, and on the east by Gumer.</obo:IAO_0000115>
        <oboInOwl:hasOBONamespace>GAZ</oboInOwl:hasOBONamespace>
        <oboInOwl:id>GAZ:00123640</oboInOwl:id>
        <rdfs:label>Enemorina Eaner Woreda</rdfs:label>
    </owl:NamedIndividual>
    


    <!-- http://purl.obolibrary.org/obo/GAZ_00123641 -->

    <owl:NamedIndividual rdf:about="http://purl.obolibrary.org/obo/GAZ_00123641">
        <obo:RO_0001025 rdf:resource="http://purl.obolibrary.org/obo/GAZ_00031146"/>
        <obo:IAO_0000115>One of the 77 woredas in the Southern Nations, Nationalities and Peoples&apos; Region of Ethiopia. Part of the Gurage Zone, Dalocha is bordered on the south by the Kembata Alaba and Tembaro Zone, on the west by the Hadiya Zone, on the north by Silte, and on the east by Lanfro. Towns in Dalocha include Dalocha, Wulbareg and Mitto.</obo:IAO_0000115>
        <oboInOwl:hasOBONamespace>GAZ</oboInOwl:hasOBONamespace>
        <oboInOwl:id>GAZ:00123641</oboInOwl:id>
        <rdfs:label>Dalocha Woreda</rdfs:label>
    </owl:NamedIndividual>
    


    <!-- http://purl.obolibrary.org/obo/GAZ_00123642 -->

    <owl:NamedIndividual rdf:about="http://purl.obolibrary.org/obo/GAZ_00123642">
        <obo:RO_0001025 rdf:resource="http://purl.obolibrary.org/obo/GAZ_00031135"/>
        <obo:IAO_0000115>One of the 77 woredas in the Southern Nations, Nationalities and Peoples&apos; Region of Ethiopia. Part of the Hadiya Zone, Konteb is bordered on the south by Soro, on the west by the Omo River which separates it from the Yem special woreda, on the north by the Hadiya Zone, and on the east by Limo. Towns in Konteb include Kose, Morsito and Sera.</obo:IAO_0000115>
        <oboInOwl:hasOBONamespace>GAZ</oboInOwl:hasOBONamespace>
        <oboInOwl:id>GAZ:00123642</oboInOwl:id>
        <rdfs:label>Konteb Woreda</rdfs:label>
    </owl:NamedIndividual>
    


    <!-- http://purl.obolibrary.org/obo/GAZ_00123643 -->

    <owl:NamedIndividual rdf:about="http://purl.obolibrary.org/obo/GAZ_00123643">
        <obo:RO_0001025 rdf:resource="http://purl.obolibrary.org/obo/GAZ_00031135"/>
        <obo:IAO_0000115>One of the 77 woredas in the Southern Nations, Nationalities and Peoples&apos; Region of Ethiopia. A triangle-shaped exclave of the Hadiya Zone, Badawacho is bordered on the south by the Semien Omo Zone, on the west and north by the Kembata Alaba and Tembaro Zone, and on the east by the Bilate River which separates it from the Oromia Region. The major town in Badawacho is Shone.</obo:IAO_0000115>
        <oboInOwl:hasOBONamespace>GAZ</oboInOwl:hasOBONamespace>
        <oboInOwl:id>GAZ:00123643</oboInOwl:id>
        <rdfs:label>Badawacho Woreda</rdfs:label>
    </owl:NamedIndividual>
    


    <!-- http://purl.obolibrary.org/obo/GAZ_00123644 -->

    <owl:NamedIndividual rdf:about="http://purl.obolibrary.org/obo/GAZ_00123644">
        <obo:RO_0001025 rdf:resource="http://purl.obolibrary.org/obo/GAZ_00031135"/>
        <obo:IAO_0000115>One of the 77 woredas in the Southern Nations, Nationalities and Peoples&apos; Region of Ethiopia. Part of the Hadiya Zone, Soro is bordered on the south and east by the Kembata Alaba and Tembaro Zone, on the west by the Omo River which separates it from the Oromia Region and the Yem special woreda, on the north by Konteb, and on the northeast by Limo. Towns in Soro include Gimbichu and Jajura.</obo:IAO_0000115>
        <oboInOwl:hasOBONamespace>GAZ</oboInOwl:hasOBONamespace>
        <oboInOwl:id>GAZ:00123644</oboInOwl:id>
        <rdfs:label>Soro Woreda</rdfs:label>
    </owl:NamedIndividual>
    


    <!-- http://purl.obolibrary.org/obo/GAZ_00123645 -->

    <owl:NamedIndividual rdf:about="http://purl.obolibrary.org/obo/GAZ_00123645">
        <obo:RO_0001025 rdf:resource="http://purl.obolibrary.org/obo/GAZ_00031135"/>
        <obo:IAO_0000115>One of the woredas in the Southern Nations, Nationalities and Peoples&apos; Region of Ethiopia. A part of the Hadiya Zone, Limo is bordered on the south and southeast by the Kembata Alaba and Tembaro Zone, on the southwest by Soro, the west by Konteb, and on the north by the Gurage Zone; most of its eastern boundary is defined by the course of the Bilate River. Towns in Lemo include Belesa, Bonosha, Do&apos;isha, Duna, Fonko, Hosaena, and Lisana.</obo:IAO_0000115>
        <oboInOwl:hasOBONamespace>GAZ</oboInOwl:hasOBONamespace>
        <oboInOwl:id>GAZ:00123645</oboInOwl:id>
        <rdfs:label>Limo Woreda</rdfs:label>
    </owl:NamedIndividual>
    


    <!-- http://purl.obolibrary.org/obo/GAZ_00123646 -->

    <owl:NamedIndividual rdf:about="http://purl.obolibrary.org/obo/GAZ_00123646">
        <obo:RO_0001025 rdf:resource="http://purl.obolibrary.org/obo/GAZ_00031134"/>
        <obo:IAO_0000115>One of the 77 woredas in the Southern Nations, Nationalities and Peoples&apos; Region of Ethiopia. Part of the Keficho Shekicho Zone, Chena is bordered on the south by the Bench Maji Zone, on the west by Yeki, on the north by Gesha, on the northeast by Ginbo, and on the southeast by Decha. Towns in Chena include Ahewa Bench, Bita Genet, Dimbira, Shishinda and Wacha.</obo:IAO_0000115>
        <oboInOwl:hasOBONamespace>GAZ</oboInOwl:hasOBONamespace>
        <oboInOwl:id>GAZ:00123646</oboInOwl:id>
        <rdfs:label>Chena Woreda</rdfs:label>
    </owl:NamedIndividual>
    


    <!-- http://purl.obolibrary.org/obo/GAZ_00123647 -->

    <owl:NamedIndividual rdf:about="http://purl.obolibrary.org/obo/GAZ_00123647">
        <obo:RO_0001025 rdf:resource="http://purl.obolibrary.org/obo/GAZ_00031134"/>
        <obo:IAO_0000115>One of the 77 woredas in the Southern Nations, Nationalities and Peoples&apos; Region of Ethiopia. Part of the Keficho Shekicho Zone, Menjiwo is bordered on the south by Telo, on the west by Ginbo, on the north by the Gojeb River which separates it from the Oromia Region, and on the east by the Semien Omo Zone. The major town in Menjiwo is Adiya Kaka.</obo:IAO_0000115>
        <oboInOwl:hasOBONamespace>GAZ</oboInOwl:hasOBONamespace>
        <oboInOwl:id>GAZ:00123647</oboInOwl:id>
        <rdfs:label>Menjiwo Woreda</rdfs:label>
    </owl:NamedIndividual>
    


    <!-- http://purl.obolibrary.org/obo/GAZ_00123648 -->

    <owl:NamedIndividual rdf:about="http://purl.obolibrary.org/obo/GAZ_00123648">
        <obo:RO_0001025 rdf:resource="http://purl.obolibrary.org/obo/GAZ_00031134"/>
        <obo:IAO_0000115>Pne of the 77 woredas in the Southern Nations, Nationalities and Peoples&apos; Region of Ethiopia. Part of the Keficho Shekicho Zone, Yeki is bordered on the south by the Bench Maji Zone, on the west by the Gambela Region, on the north by Masha Anderacha, on the northeast by Gesha, and on the east by Chena. The major town in Yeki is Tippi.</obo:IAO_0000115>
        <oboInOwl:hasOBONamespace>GAZ</oboInOwl:hasOBONamespace>
        <oboInOwl:id>GAZ:00123648</oboInOwl:id>
        <rdfs:label>Yeki Woreda</rdfs:label>
    </owl:NamedIndividual>
    


    <!-- http://purl.obolibrary.org/obo/GAZ_00123649 -->

    <owl:NamedIndividual rdf:about="http://purl.obolibrary.org/obo/GAZ_00123649">
        <obo:RO_0001025 rdf:resource="http://purl.obolibrary.org/obo/GAZ_00031134"/>
        <obo:IAO_0000115>One of the 77 woredas in the Southern Nations, Nationalities and Peoples&apos; Region of Ethiopia. Part of the Keficho Shekicho Zone, Gesha is bordered on the south by Chena, on the southwest by Yeki, on the west by Masha Anderacha, on the north by the Oromia Region, and on the east by Ginbo. Towns in Gesha include Deka and Yadeta.</obo:IAO_0000115>
        <oboInOwl:hasOBONamespace>GAZ</oboInOwl:hasOBONamespace>
        <oboInOwl:id>GAZ:00123649</oboInOwl:id>
        <rdfs:label>Gesha Woreda</rdfs:label>
    </owl:NamedIndividual>
    


    <!-- http://purl.obolibrary.org/obo/GAZ_00123650 -->

    <owl:NamedIndividual rdf:about="http://purl.obolibrary.org/obo/GAZ_00123650">
        <obo:RO_0001025 rdf:resource="http://purl.obolibrary.org/obo/GAZ_00031134"/>
        <obo:IAO_0000115>One of the 77 woredas in the Southern Nations, Nationalities and Peoples&apos; Region of Ethiopia. A triangle-shaped district of the Keficho Shekicho Zone, Telo is bordered on the on the west by Decha, at the northwest point by Ginbo, on the north by Menjiwo, and on the east by the Semien Omo Zone. Towns in Telo include Felege Selam and Shama.</obo:IAO_0000115>
        <oboInOwl:hasOBONamespace>GAZ</oboInOwl:hasOBONamespace>
        <oboInOwl:id>GAZ:00123650</oboInOwl:id>
        <rdfs:label>Telo Woreda</rdfs:label>
    </owl:NamedIndividual>
    


    <!-- http://purl.obolibrary.org/obo/GAZ_00123651 -->

    <owl:NamedIndividual rdf:about="http://purl.obolibrary.org/obo/GAZ_00123651">
        <obo:RO_0001025 rdf:resource="http://purl.obolibrary.org/obo/GAZ_00031134"/>
        <obo:IAO_0000115>One of the 77 woredas in the Southern Nations, Nationalities and Peoples&apos; Region of Ethiopia. Part of the Keficho Shekicho Zone, Ginbo is bordered on the south by Decha, on the west by Chena, on the north by the Gojeb River which separates it from the Oromia Region, on the east by Menjiwo, and on the southeast by Telo. Towns in Ginbo include Bonga, Diri, Gojeb, Keboch, Ufa and Wushwush.</obo:IAO_0000115>
        <oboInOwl:hasOBONamespace>GAZ</oboInOwl:hasOBONamespace>
        <oboInOwl:id>GAZ:00123651</oboInOwl:id>
        <rdfs:label>Ginbo Woreda</rdfs:label>
    </owl:NamedIndividual>
    


    <!-- http://purl.obolibrary.org/obo/GAZ_00123652 -->

    <owl:NamedIndividual rdf:about="http://purl.obolibrary.org/obo/GAZ_00123652">
        <obo:RO_0001025 rdf:resource="http://purl.obolibrary.org/obo/GAZ_00031134"/>
        <obo:IAO_0000115>One of the 77 woredas in the Southern Nations, Nationalities and Peoples&apos; Region of Ethiopia. Part of the Keficho Shekicho Zone, Decha is bordered on the south by the Omo River which separates it from the Debub Omo Zone, on the southwest by the Bench Maji Zone, on the northeast by Chena, on the north by Ginbo, on the northeast by Telo, and on the southeast by the Denchya River which separates it from the Semien Omo Zone. The major town in Decha is Chiri.</obo:IAO_0000115>
        <oboInOwl:hasOBONamespace>GAZ</oboInOwl:hasOBONamespace>
        <oboInOwl:id>GAZ:00123652</oboInOwl:id>
        <rdfs:label>Decha Woreda</rdfs:label>
    </owl:NamedIndividual>
    


    <!-- http://purl.obolibrary.org/obo/GAZ_00123653 -->

    <owl:NamedIndividual rdf:about="http://purl.obolibrary.org/obo/GAZ_00123653">
        <obo:RO_0001025 rdf:resource="http://purl.obolibrary.org/obo/GAZ_00031134"/>
        <obo:IAO_0000115>One of the 77 woredas in the Southern Nations, Nationalities and Peoples&apos; Region of Ethiopia. Part of the Keficho Shekicho Zone, Masha Anderacha is bordered on the south by Yeki, on the west and north by the Oromia Region, and on the east by Gesha. Towns in Masha Anderacha include Gecha and Masha, as well as the village and former capital of the Kingdom of Kaffa, Anderaccha.</obo:IAO_0000115>
        <oboInOwl:hasOBONamespace>GAZ</oboInOwl:hasOBONamespace>
        <oboInOwl:id>GAZ:00123653</oboInOwl:id>
        <rdfs:label>Masha Anderacha Woreda</rdfs:label>
    </owl:NamedIndividual>
    


    <!-- http://purl.obolibrary.org/obo/GAZ_00123654 -->

    <owl:NamedIndividual rdf:about="http://purl.obolibrary.org/obo/GAZ_00123654">
        <obo:RO_0001025 rdf:resource="http://purl.obolibrary.org/obo/GAZ_00031141"/>
        <obo:IAO_0000115>One of the 77 woredas in the Southern Nations, Nationalities and Peoples&apos; Region of Ethiopia.</obo:IAO_0000115>
        <oboInOwl:hasOBONamespace>GAZ</oboInOwl:hasOBONamespace>
        <oboInOwl:id>GAZ:00123654</oboInOwl:id>
        <rdfs:label>Damboya Woreda</rdfs:label>
    </owl:NamedIndividual>
    


    <!-- http://purl.obolibrary.org/obo/GAZ_00123655 -->

    <owl:NamedIndividual rdf:about="http://purl.obolibrary.org/obo/GAZ_00123655">
        <obo:RO_0001025 rdf:resource="http://purl.obolibrary.org/obo/GAZ_00031141"/>
        <obo:IAO_0000115>One of the 77 woredas in the Southern Nations, Nationalities and Peoples&apos; Region of Ethiopia. Part of the Kembata Alaba and Tembaro (KAT) Zone, Kedida Gamela is bordered on the south by an exclave of the Hadiya Zone, on the southwest by Kacha Bira, on the west by Angacha, on the north by the Hadiya Zone, and on the east by the Bilate River which separates it from Alaba. The admnistrative center for the KAT is Durame; other towns in Kedida Gamela include Damboya.</obo:IAO_0000115>
        <oboInOwl:hasOBONamespace>GAZ</oboInOwl:hasOBONamespace>
        <oboInOwl:id>GAZ:00123655</oboInOwl:id>
        <rdfs:label>Kedida Gamela Woreda</rdfs:label>
    </owl:NamedIndividual>
    


    <!-- http://purl.obolibrary.org/obo/GAZ_00123656 -->

    <owl:NamedIndividual rdf:about="http://purl.obolibrary.org/obo/GAZ_00123656">
        <obo:RO_0001025 rdf:resource="http://purl.obolibrary.org/obo/GAZ_00031141"/>
        <obo:IAO_0000115>One of the 77 woredas in the Southern Nations, Nationalities and Peoples&apos; Region of Ethiopia.</obo:IAO_0000115>
        <oboInOwl:hasOBONamespace>GAZ</oboInOwl:hasOBONamespace>
        <oboInOwl:id>GAZ:00123656</oboInOwl:id>
        <rdfs:label>Haderona Tunto Zuria Woreda</rdfs:label>
    </owl:NamedIndividual>
    


    <!-- http://purl.obolibrary.org/obo/GAZ_00123657 -->

    <owl:NamedIndividual rdf:about="http://purl.obolibrary.org/obo/GAZ_00123657">
        <obo:RO_0001025 rdf:resource="http://purl.obolibrary.org/obo/GAZ_00031141"/>
        <obo:IAO_0000115>One of the 77 woredas in the Southern Nations, Nationalities and Peoples&apos; Region of Ethiopia. Part of the Kembata Alaba and Tembaro Zone, Angacha is bordered on the south by Kacha Bira, on the west and north by the Hadiya Zone, and on the east by Kedida Gamela. Towns in Angacha include Angacha and Deyogena.</obo:IAO_0000115>
        <oboInOwl:hasOBONamespace>GAZ</oboInOwl:hasOBONamespace>
        <oboInOwl:id>GAZ:00123657</oboInOwl:id>
        <rdfs:label>Angacha Woreda</rdfs:label>
    </owl:NamedIndividual>
    


    <!-- http://purl.obolibrary.org/obo/GAZ_00123658 -->

    <owl:NamedIndividual rdf:about="http://purl.obolibrary.org/obo/GAZ_00123658">
        <obo:RO_0001025 rdf:resource="http://purl.obolibrary.org/obo/GAZ_00031141"/>
        <obo:IAO_0000115>One of the 77 woredas in the Southern Nations, Nationalities and Peoples&apos; Region of Ethiopia.</obo:IAO_0000115>
        <oboInOwl:hasOBONamespace>GAZ</oboInOwl:hasOBONamespace>
        <oboInOwl:id>GAZ:00123658</oboInOwl:id>
        <rdfs:label>Tembaro Woreda</rdfs:label>
    </owl:NamedIndividual>
    


    <!-- http://purl.obolibrary.org/obo/GAZ_00123659 -->

    <owl:NamedIndividual rdf:about="http://purl.obolibrary.org/obo/GAZ_00123659">
        <obo:RO_0001025 rdf:resource="http://purl.obolibrary.org/obo/GAZ_00031141"/>
        <obo:IAO_0000115>One of the 77 woredas in the Southern Nations, Nationalities and Peoples&apos; Region of Ethiopia.</obo:IAO_0000115>
        <oboInOwl:hasOBONamespace>GAZ</oboInOwl:hasOBONamespace>
        <oboInOwl:id>GAZ:00123659</oboInOwl:id>
        <rdfs:label>Doyogena Woreda</rdfs:label>
    </owl:NamedIndividual>
    


    <!-- http://purl.obolibrary.org/obo/GAZ_00123660 -->

    <owl:NamedIndividual rdf:about="http://purl.obolibrary.org/obo/GAZ_00123660">
        <obo:RO_0001025 rdf:resource="http://purl.obolibrary.org/obo/GAZ_00031141"/>
        <obo:IAO_0000115>One of the 77 woredas in the Southern Nations, Nationalities and Peoples&apos; Region of Ethiopia. Part of the Kembata Alaba and Tembaro Zone, Kacha Bira is bordered on the south by an exclave of the Hadiya Zone, on the southwest by the Semien Omo Zone, on the west by Omo Sheleko, on the northwest by the Hadiya Zone, on the north by Angacha, and on the east by Alaba. Towns in Kacha Bira include Shinshicho and Hadero.</obo:IAO_0000115>
        <oboInOwl:hasOBONamespace>GAZ</oboInOwl:hasOBONamespace>
        <oboInOwl:id>GAZ:00123660</oboInOwl:id>
        <rdfs:label>Kacha Bira Woreda</rdfs:label>
    </owl:NamedIndividual>
    


    <!-- http://purl.obolibrary.org/obo/GAZ_00123661 -->

    <owl:NamedIndividual rdf:about="http://purl.obolibrary.org/obo/GAZ_00123661">
        <obo:RO_0001025 rdf:resource="http://purl.obolibrary.org/obo/GAZ_00031145"/>
        <obo:IAO_0000115>One of the 77 woredas in the Southern Nations, Nationalities and Peoples&apos; Region of Ethiopia. Part of the Semien Omo Zone, Bonke is bordered on the south by the Dirashe special woreda, on the west by the Weito River which separates it from Kemba, on the north by Dita Dermalo, and on the east by Arba Minch Zuria. The major town in Bonke is Gerese.</obo:IAO_0000115>
        <oboInOwl:hasOBONamespace>GAZ</oboInOwl:hasOBONamespace>
        <oboInOwl:id>GAZ:00123661</oboInOwl:id>
        <rdfs:label>Bonke Woreda</rdfs:label>
    </owl:NamedIndividual>
    


    <!-- http://purl.obolibrary.org/obo/GAZ_00123662 -->

    <owl:NamedIndividual rdf:about="http://purl.obolibrary.org/obo/GAZ_00123662">
        <obo:RO_0001025 rdf:resource="http://purl.obolibrary.org/obo/GAZ_00031145"/>
        <obo:IAO_0000115>One of the 77 woredas in the Southern Nations, Nationalities and Peoples&apos; Region of Ethiopia. Part of the Semien Omo Zone, Zala Ubamale is bordered on the south and west by the Debub Omo Zone, on the northwest by Gofa Zuria, on the northeast by Kucha, on the east by Dita Dermalo and on the southeast by Kemba. Towns in Zala Ubamale include Beto and Meleante.</obo:IAO_0000115>
        <oboInOwl:hasOBONamespace>GAZ</oboInOwl:hasOBONamespace>
        <oboInOwl:id>GAZ:00123662</oboInOwl:id>
        <rdfs:label>Zala Ubamale Woreda</rdfs:label>
    </owl:NamedIndividual>
    


    <!-- http://purl.obolibrary.org/obo/GAZ_00123663 -->

    <owl:NamedIndividual rdf:about="http://purl.obolibrary.org/obo/GAZ_00123663">
        <obo:RO_0001025 rdf:resource="http://purl.obolibrary.org/obo/GAZ_00031145"/>
        <obo:IAO_0000115>One of the 77 woredas in the Southern Nations, Nationalities and Peoples&apos; Region of Ethiopia. Basketo is bordered on the south and west by the Debub Omo Zone, on the north by Melokoza, and on the east by Gofa Zuria. The major town in Basketo is Laska.</obo:IAO_0000115>
        <oboInOwl:hasOBONamespace>GAZ</oboInOwl:hasOBONamespace>
        <oboInOwl:id>GAZ:00123663</oboInOwl:id>
        <rdfs:label>Basketo Woreda</rdfs:label>
    </owl:NamedIndividual>
    


    <!-- http://purl.obolibrary.org/obo/GAZ_00123664 -->

    <owl:NamedIndividual rdf:about="http://purl.obolibrary.org/obo/GAZ_00123664">
        <obo:RO_0001025 rdf:resource="http://purl.obolibrary.org/obo/GAZ_00031145"/>
        <obo:IAO_0000115>One of the 77 woredas in the Southern Nations, Nationalities and Peoples&apos; Region of Ethiopia. Part of the Semien Omo Zone, Kemba is bordered on the southwest by the Debub Omo Zone, on the west by Zala Ubamale, on the north by Dita Dermalo, on the east by Bonke, and on the southeast by the Dirashe special woreda; the Weito River defines the boundary with Bonke and Dirashe. The major town in Kemba is Kemba.</obo:IAO_0000115>
        <oboInOwl:hasOBONamespace>GAZ</oboInOwl:hasOBONamespace>
        <oboInOwl:id>GAZ:00123664</oboInOwl:id>
        <rdfs:label>Kemba Woreda</rdfs:label>
    </owl:NamedIndividual>
    


    <!-- http://purl.obolibrary.org/obo/GAZ_00123665 -->

    <owl:NamedIndividual rdf:about="http://purl.obolibrary.org/obo/GAZ_00123665">
        <obo:RO_0001025 rdf:resource="http://purl.obolibrary.org/obo/GAZ_00031145"/>
        <obo:IAO_0000115>One of the 77 woredas in the Southern Nations, Nationalities and Peoples&apos; Region of Ethiopia. Part of the Semien Omo Zone located in the Great Rift Valley, Damot Weyde is bordered on the south by Humbo, on the west by Sodo Zuria, on the northwest by Damot Gale, on the north by the Hadiya Zone, on the northeast by the Oromia Region, and on the east by the Bilate River which separates it from the Sidama Zone. Towns in Damot Weyde include Bedesa and Dimtu.</obo:IAO_0000115>
        <oboInOwl:hasOBONamespace>GAZ</oboInOwl:hasOBONamespace>
        <oboInOwl:id>GAZ:00123665</oboInOwl:id>
        <rdfs:label>Damot Weyde Woreda</rdfs:label>
    </owl:NamedIndividual>
    


    <!-- http://purl.obolibrary.org/obo/GAZ_00123666 -->

    <owl:NamedIndividual rdf:about="http://purl.obolibrary.org/obo/GAZ_00123666">
        <obo:RO_0001025 rdf:resource="http://purl.obolibrary.org/obo/GAZ_00031145"/>
        <obo:IAO_0000115>One of the 77 woredas in the Southern Nations, Nationalities and Peoples&apos; Region of Ethiopia. Part of the Semien Omo Zone, Gofa Zuria is bordered on the south by Zala Ubamale, on the southwest by the Debub Omo Zone, on the west by Basketo, on the northwest by Melokoza, on the north by Loma Bosa, and on the east by Kucha. The administrative center of Gofa Zuria is Bulki; other towns include Sawla.</obo:IAO_0000115>
        <oboInOwl:hasOBONamespace>GAZ</oboInOwl:hasOBONamespace>
        <oboInOwl:id>GAZ:00123666</oboInOwl:id>
        <rdfs:label>Gofa Zuria Woreda</rdfs:label>
    </owl:NamedIndividual>
    


    <!-- http://purl.obolibrary.org/obo/GAZ_00123667 -->

    <owl:NamedIndividual rdf:about="http://purl.obolibrary.org/obo/GAZ_00123667">
        <obo:RO_0001025 rdf:resource="http://purl.obolibrary.org/obo/GAZ_00031145"/>
        <obo:IAO_0000115>One of the 77 woredas in the Southern Nations, Nationalities and Peoples&apos; Region of Ethiopia. Part of the Semien Omo Zone, Dita Dermalo is bordered on the south by Bonke, on the southwest by Kemba, on the west by Zala Ubamale, on the north by Kucha, and on the east by Chencha. Towns in Dita Dermalo include Wacha and Zeda.</obo:IAO_0000115>
        <oboInOwl:hasOBONamespace>GAZ</oboInOwl:hasOBONamespace>
        <oboInOwl:id>GAZ:00123667</oboInOwl:id>
        <rdfs:label>Dita Dermalo Woreda</rdfs:label>
    </owl:NamedIndividual>
    


    <!-- http://purl.obolibrary.org/obo/GAZ_00123668 -->

    <owl:NamedIndividual rdf:about="http://purl.obolibrary.org/obo/GAZ_00123668">
        <obo:RO_0001025 rdf:resource="http://purl.obolibrary.org/obo/GAZ_00031145"/>
        <obo:IAO_0000115>One of the 77 woredas in the Southern Nations, Nationalities and Peoples&apos; Region of Ethiopia. Part of the Semien Omo Zone, Kucha is bordered on the south by Dita Dermalo, on the southwest by Zala Ubamale, on the west by Gofa Zuria, on the northwest by Loma Bosa, on the north by Offa, on the east by Boreda Abaya, and on the southeast by Chencha. The major town in Kucha is Selamber.</obo:IAO_0000115>
        <oboInOwl:hasOBONamespace>GAZ</oboInOwl:hasOBONamespace>
        <oboInOwl:id>GAZ:00123668</oboInOwl:id>
        <rdfs:label>Kucha Woreda</rdfs:label>
    </owl:NamedIndividual>
    


    <!-- http://purl.obolibrary.org/obo/GAZ_00123669 -->

    <owl:NamedIndividual rdf:about="http://purl.obolibrary.org/obo/GAZ_00123669">
        <obo:RO_0001025 rdf:resource="http://purl.obolibrary.org/obo/GAZ_00031145"/>
        <obo:IAO_0000115>One of the 77 woredas in the Southern Nations, Nationalities and Peoples&apos; Region of Ethiopia. Part of the Semien Omo Zone, Chencha is bordered on the south by Arba Minch Zuria, on the west by Dita Dermalo, on the north by Kucha, and on the east by Boreda Abaya. Towns in Chencha include Chencha, Dorze and Ezo.</obo:IAO_0000115>
        <oboInOwl:hasOBONamespace>GAZ</oboInOwl:hasOBONamespace>
        <oboInOwl:id>GAZ:00123669</oboInOwl:id>
        <rdfs:label>Chencha Woreda</rdfs:label>
    </owl:NamedIndividual>
    


    <!-- http://purl.obolibrary.org/obo/GAZ_00123670 -->

    <owl:NamedIndividual rdf:about="http://purl.obolibrary.org/obo/GAZ_00123670">
        <obo:RO_0001025 rdf:resource="http://purl.obolibrary.org/obo/GAZ_00031145"/>
        <obo:IAO_0000115>One of the 77 woredas in the Southern Nations, Nationalities and Peoples&apos; Region of Ethiopia. Part of the Semien Omo Zone, Isara Tocha is bordered on the south by the Omo River which separates this woreda from Melokoza, on the west by Ela, on the north by the Gojeb River which separates it from the Oromia Region, on the east by Mareka Gena, and on the southeast by Loma Bosa. Towns in Isara Tocha include Bale and Tocha.</obo:IAO_0000115>
        <oboInOwl:hasOBONamespace>GAZ</oboInOwl:hasOBONamespace>
        <oboInOwl:id>GAZ:00123670</oboInOwl:id>
        <rdfs:label>Isara Tocha Woreda</rdfs:label>
    </owl:NamedIndividual>
    


    <!-- http://purl.obolibrary.org/obo/GAZ_00123671 -->

    <owl:NamedIndividual rdf:about="http://purl.obolibrary.org/obo/GAZ_00123671">
        <obo:RO_0001025 rdf:resource="http://purl.obolibrary.org/obo/GAZ_00031145"/>
        <obo:IAO_0000115>One of the 77 woredas in the Southern Nations, Nationalities and Peoples&apos; Region of Ethiopia. Part of the Semien Omo Zone, Ela is bordered on the south by the Omo River which separates it from Melokoza, on the west by the Keficho Shekicho Zone, on the north by the Gojeb River which separates it from the Oromia Zone, and on the east by Isara Tocha; the Denchya River defines the southern part of the boundary with the Keficho Shekicho Zone. Towns in Ela include Ameya and Chida.</obo:IAO_0000115>
        <oboInOwl:hasOBONamespace>GAZ</oboInOwl:hasOBONamespace>
        <oboInOwl:id>GAZ:00123671</oboInOwl:id>
        <rdfs:label>Ela Woreda</rdfs:label>
    </owl:NamedIndividual>
    


    <!-- http://purl.obolibrary.org/obo/GAZ_00123672 -->

    <owl:NamedIndividual rdf:about="http://purl.obolibrary.org/obo/GAZ_00123672">
        <obo:RO_0001025 rdf:resource="http://purl.obolibrary.org/obo/GAZ_00031145"/>
        <obo:IAO_0000115>One of the 77 woredas in the Southern Nations, Nationalities and Peoples&apos; Region of Ethiopia. Part of the Semien Omo Zone, Kindo Koysha is bordered on the south by Offa, on the west by Loma Bosa, on the north by Boloso Sore, and on the east by Sodo Zuria. The major town in Kindo Koysha is Bele.</obo:IAO_0000115>
        <oboInOwl:hasOBONamespace>GAZ</oboInOwl:hasOBONamespace>
        <oboInOwl:id>GAZ:00123672</oboInOwl:id>
        <rdfs:label>Kindo Koysha Woreda</rdfs:label>
    </owl:NamedIndividual>
    


    <!-- http://purl.obolibrary.org/obo/GAZ_00123673 -->

    <owl:NamedIndividual rdf:about="http://purl.obolibrary.org/obo/GAZ_00123673">
        <obo:RO_0001025 rdf:resource="http://purl.obolibrary.org/obo/GAZ_00031145"/>
        <obo:IAO_0000115>One of the 77 woredas in the Southern Nations, Nationalities and Peoples&apos; Region of Ethiopia. Part of the Semien Omo Zone, Damot Gale is bordered on the south by Sodo Zuria, on the west by Boloso Sore, on the north by the Hadiya Zone, and on the east by Damot Weyde. The major town in Damot Gale is Boditi.</obo:IAO_0000115>
        <oboInOwl:hasOBONamespace>GAZ</oboInOwl:hasOBONamespace>
        <oboInOwl:id>GAZ:00123673</oboInOwl:id>
        <rdfs:label>Damot Gale Woreda</rdfs:label>
    </owl:NamedIndividual>
    


    <!-- http://purl.obolibrary.org/obo/GAZ_00123674 -->

    <owl:NamedIndividual rdf:about="http://purl.obolibrary.org/obo/GAZ_00123674">
        <obo:RO_0001025 rdf:resource="http://purl.obolibrary.org/obo/GAZ_00031145"/>
        <obo:IAO_0000115>One of the 77 woredas in the Southern Nations, Nationalities and Peoples&apos; Region of Ethiopia. Part of the Semien Omo Zone, Loma Bosa is bordered on the south by Gofa Zuria, on the southwest by Melokoza, on the west by Isara Tocha, on the northwest by Mareka Gena, on the north by the Kembata Alaba and Tembaro Zone, on the northeast by Boloso Sore, on the east by Kindo Koysha, and on the southeast by Offa; the Omo River defines Loma Bose&apos;s boundary on the northeast, east and south.</obo:IAO_0000115>
        <oboInOwl:hasOBONamespace>GAZ</oboInOwl:hasOBONamespace>
        <oboInOwl:id>GAZ:00123674</oboInOwl:id>
        <rdfs:label>Loma Bosa Woreda</rdfs:label>
    </owl:NamedIndividual>
    


    <!-- http://purl.obolibrary.org/obo/GAZ_00123675 -->

    <owl:NamedIndividual rdf:about="http://purl.obolibrary.org/obo/GAZ_00123675">
        <obo:RO_0001025 rdf:resource="http://purl.obolibrary.org/obo/GAZ_00031145"/>
        <obo:IAO_0000115>One of the 77 woredas in the Southern Nations, Nationalities and Peoples&apos; Region of Ethiopia. Part of the Semien Omo Zone located in the Great Rift Valley, Humbo is bordered on the south by Lake Abaya which separates it from the Oromia Region, on the southwest by Boreda Abaya, on the west by Offa, on the north by Sodo Zuria, on the northeast by Damot Weyde, and on the east by the Bilate River which separates it from the Sidama Zone. The major town in Humbo is Tebela.</obo:IAO_0000115>
        <oboInOwl:hasOBONamespace>GAZ</oboInOwl:hasOBONamespace>
        <oboInOwl:id>GAZ:00123675</oboInOwl:id>
        <rdfs:label>Humbo Woreda</rdfs:label>
    </owl:NamedIndividual>
    


    <!-- http://purl.obolibrary.org/obo/GAZ_00123676 -->

    <owl:NamedIndividual rdf:about="http://purl.obolibrary.org/obo/GAZ_00123676">
        <obo:RO_0001025 rdf:resource="http://purl.obolibrary.org/obo/GAZ_00031145"/>
        <obo:IAO_0000115>One of the 77 woredas in the Southern Nations, Nationalities and Peoples&apos; Region of Ethiopia. Part of the Semien Omo Zone, Boloso Sore is bordered on the south by Sodo Zuria, on the southwest by Kindo Koysha, on the west by Loma Bosa, on the north by the Kembata Alaba and Tembaro Zone, on the northeast by the Hadiya Zone, and on the east by Damot Gale. Towns in Boloso Sore include Areka, Bombe Edget and Gununo Hamus Edget.</obo:IAO_0000115>
        <oboInOwl:hasOBONamespace>GAZ</oboInOwl:hasOBONamespace>
        <oboInOwl:id>GAZ:00123676</oboInOwl:id>
        <rdfs:label>Boloso Sore Woreda</rdfs:label>
    </owl:NamedIndividual>
    


    <!-- http://purl.obolibrary.org/obo/GAZ_00123677 -->

    <owl:NamedIndividual rdf:about="http://purl.obolibrary.org/obo/GAZ_00123677">
        <obo:RO_0001025 rdf:resource="http://purl.obolibrary.org/obo/GAZ_00031145"/>
        <obo:IAO_0000115>One of the 77 woredas in the Southern Nations, Nationalities and Peoples&apos; Region of Ethiopia. Part of the Semien Omo Zone, Sodo Zuria is bordered on the southwest by Offa, on the west by Kindo Koysha, on the north by Boloso Sore, on the northeast by Damot Gale, and on the east by Damot Weyde. The major town in Sodo Zuria is Sodo.</obo:IAO_0000115>
        <oboInOwl:hasOBONamespace>GAZ</oboInOwl:hasOBONamespace>
        <oboInOwl:id>GAZ:00123677</oboInOwl:id>
        <rdfs:label>Sodo Zuria Woreda</rdfs:label>
    </owl:NamedIndividual>
    


    <!-- http://purl.obolibrary.org/obo/GAZ_00123678 -->

    <owl:NamedIndividual rdf:about="http://purl.obolibrary.org/obo/GAZ_00123678">
        <obo:RO_0001025 rdf:resource="http://purl.obolibrary.org/obo/GAZ_00031145"/>
        <obo:IAO_0000115>One of the 77 woredas in the Southern Nations, Nationalities and Peoples&apos; Region of Ethiopia. Part of the Semien Omo Zone, Offa is bordered on the south by Kucha, on the west by Loma Bosa, on the northwest by Kindo Koysha, on the northeast by Sodo Zuria, and on the east by Humbo. The major town in Offa is Gesuba.</obo:IAO_0000115>
        <oboInOwl:hasOBONamespace>GAZ</oboInOwl:hasOBONamespace>
        <oboInOwl:id>GAZ:00123678</oboInOwl:id>
        <rdfs:label>Offa Woreda</rdfs:label>
    </owl:NamedIndividual>
    


    <!-- http://purl.obolibrary.org/obo/GAZ_00123679 -->

    <owl:NamedIndividual rdf:about="http://purl.obolibrary.org/obo/GAZ_00123679">
        <obo:RO_0001025 rdf:resource="http://purl.obolibrary.org/obo/GAZ_00031145"/>
        <obo:IAO_0000115>One of the 77 woredas in the Southern Nations, Nationalities and Peoples&apos; Region of Ethiopia. Part of the Semien Omo Zone, Melokoza is bordered on the south by Basketo, on the west by the Debub Omo Zone, on the northwest by Ela, on the north by Isara Tocha, and on the east by Loma Bosa; the Omo River defines its northwestern boundary separating the woreda from Ela and Isara Tocha. The major town in Melokoza is Leha.</obo:IAO_0000115>
        <oboInOwl:hasOBONamespace>GAZ</oboInOwl:hasOBONamespace>
        <oboInOwl:id>GAZ:00123679</oboInOwl:id>
        <rdfs:label>Melokoza Woreda</rdfs:label>
    </owl:NamedIndividual>
    


    <!-- http://purl.obolibrary.org/obo/GAZ_00123680 -->

    <owl:NamedIndividual rdf:about="http://purl.obolibrary.org/obo/GAZ_00123680">
        <obo:RO_0001025 rdf:resource="http://purl.obolibrary.org/obo/GAZ_00031145"/>
        <obo:IAO_0000115>One of the 77 woredas in the Southern Nations, Nationalities and Peoples&apos; Region of Ethiopia. Part of the Semien Omo Zone, Boreda Abaya is bordered on the south by Arba Minch Zuria, on the southwest by Chencha, on the west by Kucha, on the north by Humbo, and on the east by Lake Abaya which separates it from the Oromia Region. Towns in Boreda Abaya include Birbir and Zefene.</obo:IAO_0000115>
        <oboInOwl:hasOBONamespace>GAZ</oboInOwl:hasOBONamespace>
        <oboInOwl:id>GAZ:00123680</oboInOwl:id>
        <rdfs:label>Boreda Abaya Woreda</rdfs:label>
    </owl:NamedIndividual>
    


    <!-- http://purl.obolibrary.org/obo/GAZ_00123681 -->

    <owl:NamedIndividual rdf:about="http://purl.obolibrary.org/obo/GAZ_00123681">
        <obo:RO_0001025 rdf:resource="http://purl.obolibrary.org/obo/GAZ_00031145"/>
        <obo:IAO_0000115>One of the 77 woredas in the Southern Nations, Nationalities and Peoples&apos; Region of Ethiopia. A part of the Semien Omo Zone located in the Great Rift Valley, Arba Minch Zuria is bordered on the south by the Dirashe special woreda, on the west by Bonke, on the north by Chencha, on the northeast by Boreda Abaya, on the east by the Oromia Region, and on the southeast by the Amaro special woreda. This woreda also includes portions of two lakes and their islands, Abaya and Chamo. The largest settlement in Arba Minch Zuria is the city of Arba Minch.</obo:IAO_0000115>
        <oboInOwl:hasOBONamespace>GAZ</oboInOwl:hasOBONamespace>
        <oboInOwl:id>GAZ:00123681</oboInOwl:id>
        <rdfs:label>Arba Minch Zuria Woreda</rdfs:label>
    </owl:NamedIndividual>
    


    <!-- http://purl.obolibrary.org/obo/GAZ_00123682 -->

    <owl:NamedIndividual rdf:about="http://purl.obolibrary.org/obo/GAZ_00123682">
        <obo:RO_0001025 rdf:resource="http://purl.obolibrary.org/obo/GAZ_00031145"/>
        <obo:IAO_0000115>One of the 77 woredas in the Southern Nations, Nationalities and Peoples&apos; Region of Ethiopia. Part of the Semien Omo Zone, Mareka Gena is a triangle-shaped area located south of the confluence of the Omo River and its east-flowing tributary the Gojeb River, bordered on the southeast by Loma Bosa, on the west by Isara Tocha, and on the north by the Oromia Region. Towns in Mareka Gena include Waka and Weldehane.</obo:IAO_0000115>
        <oboInOwl:hasOBONamespace>GAZ</oboInOwl:hasOBONamespace>
        <oboInOwl:id>GAZ:00123682</oboInOwl:id>
        <rdfs:label>Mareka Gena Woreda</rdfs:label>
    </owl:NamedIndividual>
    


    <!-- http://purl.obolibrary.org/obo/GAZ_00123683 -->

    <owl:NamedIndividual rdf:about="http://purl.obolibrary.org/obo/GAZ_00123683">
        <obo:RO_0001025 rdf:resource="http://purl.obolibrary.org/obo/GAZ_00031143"/>
        <obo:IAO_0000115>One of the 77 woredas in the Southern Nations, Nationalities and Peoples&apos; Region of Ethiopia. Part of the Debub Omo Zone, Bako Gazer is bordered on the south by Hamer Bena, on the west by the Mago River which separates it from Selamago, and on the north by the Semien Omo Zone, and on the east by the Weito River which separates it from the Dirashe special woreda; part of the southern boundary is defined by the Neri River. Towns in Bako Gazer include Jinka, Tolta and Wub Hamer.</obo:IAO_0000115>
        <oboInOwl:hasOBONamespace>GAZ</oboInOwl:hasOBONamespace>
        <oboInOwl:id>GAZ:00123683</oboInOwl:id>
        <rdfs:label>Bako Gazer Woreda</rdfs:label>
    </owl:NamedIndividual>
    


    <!-- http://purl.obolibrary.org/obo/GAZ_00123684 -->

    <owl:NamedIndividual rdf:about="http://purl.obolibrary.org/obo/GAZ_00123684">
        <obo:RO_0001025 rdf:resource="http://purl.obolibrary.org/obo/GAZ_00031143"/>
        <obo:IAO_0000115>A woreda in the extreme south of Ethiopia. Part of the Debub Omo Zone of the Southern Nations, Nationalities and Peoples&apos; Region, Kuraz is bordered on the south by Kenya, on the west by the Ilemi Triangle (claimed by Ethiopia, Kenya and Sudan), on the north by Selamago, and on the east by the Omo River which separates it from Hamer Bena. The only town in this woreda is Omorate.</obo:IAO_0000115>
        <oboInOwl:hasOBONamespace>GAZ</oboInOwl:hasOBONamespace>
        <oboInOwl:id>GAZ:00123684</oboInOwl:id>
        <rdfs:label>Kuraz Woreda</rdfs:label>
    </owl:NamedIndividual>
    


    <!-- http://purl.obolibrary.org/obo/GAZ_00123685 -->

    <owl:NamedIndividual rdf:about="http://purl.obolibrary.org/obo/GAZ_00123685">
        <obo:RO_0001025 rdf:resource="http://purl.obolibrary.org/obo/GAZ_00031143"/>
        <obo:IAO_0000115>One of the 77 woredas in the Southern Nations, Nationalities and Peoples&apos; Region of Ethiopia. Part of the Debub Omo Zone, Selamago is bordered on the south by Kuraz, on the west by the Omo River which separates it from the Bench Maji Zone and the Keficho Shekicho Zone, on the north by the Semien Omo Zone, on the east by Bako Gazer, and on the southeast by the Usno River which separates it from Hamer Bena; the Mago River defines part of the boundary with Bako Gazer. The major town in Selamago is Hana.</obo:IAO_0000115>
        <oboInOwl:hasOBONamespace>GAZ</oboInOwl:hasOBONamespace>
        <oboInOwl:id>GAZ:00123685</oboInOwl:id>
        <rdfs:label>Selamago Woreda</rdfs:label>
    </owl:NamedIndividual>
    


    <!-- http://purl.obolibrary.org/obo/GAZ_00123686 -->

    <owl:NamedIndividual rdf:about="http://purl.obolibrary.org/obo/GAZ_00123686">
        <obo:RO_0001025 rdf:resource="http://purl.obolibrary.org/obo/GAZ_00031139"/>
        <obo:IAO_0000115>One of the 77 woredas in the Southern Nations, Nationalities and Peoples&apos; Region of Ethiopia. Part of the Sidama Zone located in the Great Rift Valley, Dale is bordered on the south by the Oromia Region, on the west by the Bilate River which separates it from the Semien Omo Zone, on the north by Shebedino, on the east by Arbegona and Hula, and on the southeast by Aleta Wendo. The major town in Dale is Irgalem.</obo:IAO_0000115>
        <oboInOwl:hasOBONamespace>GAZ</oboInOwl:hasOBONamespace>
        <oboInOwl:id>GAZ:00123686</oboInOwl:id>
        <rdfs:label>Dale Woreda</rdfs:label>
    </owl:NamedIndividual>
    


    <!-- http://purl.obolibrary.org/obo/GAZ_00123687 -->

    <owl:NamedIndividual rdf:about="http://purl.obolibrary.org/obo/GAZ_00123687">
        <obo:RO_0001025 rdf:resource="http://purl.obolibrary.org/obo/GAZ_00031139"/>
        <obo:IAO_0000115>One of the 77 woredas in the Southern Nations, Nationalities and Peoples&apos; Region of Ethiopia. Part of the Sidama Zone located in the Great Rift Valley, Shebedino is bordered on the south by Dale, on the west by the Bilate River which separates it from the Semien Omo Zone, on the northwest by the Oromia Region, on the north by Awasa, and on the southeast by Arbegona.</obo:IAO_0000115>
        <oboInOwl:hasOBONamespace>GAZ</oboInOwl:hasOBONamespace>
        <oboInOwl:id>GAZ:00123687</oboInOwl:id>
        <rdfs:label>Shebedino Woreda</rdfs:label>
    </owl:NamedIndividual>
    


    <!-- http://purl.obolibrary.org/obo/GAZ_00123688 -->

    <owl:NamedIndividual rdf:about="http://purl.obolibrary.org/obo/GAZ_00123688">
        <obo:RO_0001025 rdf:resource="http://purl.obolibrary.org/obo/GAZ_00031139"/>
        <obo:IAO_0000115>One of the 77 woredas in the Southern Nations, Nationalities and Peoples&apos; Region of Ethiopia. Part of the Sidama Zone, Dara is bordered on the south by the Gedeo Zone and on either side of it by the Oromia Region, on the northwest by Aleta Wendo, and on the northeast by Hula. Towns in Dara include Kebado and Teferi Kela.</obo:IAO_0000115>
        <oboInOwl:hasOBONamespace>GAZ</oboInOwl:hasOBONamespace>
        <oboInOwl:id>GAZ:00123688</oboInOwl:id>
        <rdfs:label>Dara Woreda</rdfs:label>
    </owl:NamedIndividual>
    


    <!-- http://purl.obolibrary.org/obo/GAZ_00123689 -->

    <owl:NamedIndividual rdf:about="http://purl.obolibrary.org/obo/GAZ_00123689">
        <obo:RO_0001025 rdf:resource="http://purl.obolibrary.org/obo/GAZ_00031139"/>
        <obo:IAO_0000115>One of the 77 woredas in the Southern Nations, Nationalities and Peoples&apos; Region of Ethiopia. Part of the Sidama Zone, Arbegona is bordered on the southwest by Hula, on the west by Dale, on the northwest by Shebedino, on the north by the Oromia Region, and on the east by Bensa. The major town in Arbegona is Arbegona.</obo:IAO_0000115>
        <oboInOwl:hasOBONamespace>GAZ</oboInOwl:hasOBONamespace>
        <oboInOwl:id>GAZ:00123689</oboInOwl:id>
        <rdfs:label>Arbegona Woreda</rdfs:label>
    </owl:NamedIndividual>
    


    <!-- http://purl.obolibrary.org/obo/GAZ_00123690 -->

    <owl:NamedIndividual rdf:about="http://purl.obolibrary.org/obo/GAZ_00123690">
        <obo:RO_0001025 rdf:resource="http://purl.obolibrary.org/obo/GAZ_00031139"/>
        <obo:IAO_0000115>One of the 77 woredas in the Southern Nations, Nationalities and Peoples&apos; Region of Ethiopia. Located at the tip of the Sidama Zone that extends into the Oromia Region like a peninsula, Aroresa is bordered on every side by that Region, except on the west where it is bordered by Bensa. The major town in Aroresa is Mejo.</obo:IAO_0000115>
        <oboInOwl:hasOBONamespace>GAZ</oboInOwl:hasOBONamespace>
        <oboInOwl:id>GAZ:00123690</oboInOwl:id>
        <rdfs:label>Aroresa Woreda</rdfs:label>
    </owl:NamedIndividual>
    


    <!-- http://purl.obolibrary.org/obo/GAZ_00123691 -->

    <owl:NamedIndividual rdf:about="http://purl.obolibrary.org/obo/GAZ_00123691">
        <obo:RO_0001025 rdf:resource="http://purl.obolibrary.org/obo/GAZ_00031139"/>
        <obo:IAO_0000115>One of the 77 woredas in the Southern Nations, Nationalities and Peoples&apos; Region of Ethiopia. Part of the Sidama Zone, Hula is bordered on the south by the Oromia Region, on the southwest by Dara, on the west by Aleta Wendo, on the northwest by Dale, on the north by Shebedino, on the northeast by Arbegona, and on the east by Bensa. The major town in Hula is Hagere Selam.</obo:IAO_0000115>
        <oboInOwl:hasOBONamespace>GAZ</oboInOwl:hasOBONamespace>
        <oboInOwl:id>GAZ:00123691</oboInOwl:id>
        <rdfs:label>Hula Woreda</rdfs:label>
    </owl:NamedIndividual>
    


    <!-- http://purl.obolibrary.org/obo/GAZ_00123692 -->

    <owl:NamedIndividual rdf:about="http://purl.obolibrary.org/obo/GAZ_00123692">
        <obo:RO_0001025 rdf:resource="http://purl.obolibrary.org/obo/GAZ_00031139"/>
        <obo:IAO_0000115>One of the 77 woredas in the Southern Nations, Nationalities and Peoples&apos; Region of Ethiopia. Part of the Sidama Zone, Aleta Wendo is bordered on the south by the Oromia Region, on the west and north by Dale, on the east by Hula, and on the southeast by Dara. The administrative center is Aleta Wendo; other towns include Chuko.</obo:IAO_0000115>
        <oboInOwl:hasOBONamespace>GAZ</oboInOwl:hasOBONamespace>
        <oboInOwl:id>GAZ:00123692</oboInOwl:id>
        <rdfs:label>Aleta Wendo Woreda</rdfs:label>
    </owl:NamedIndividual>
    


    <!-- http://purl.obolibrary.org/obo/GAZ_00123693 -->

    <owl:NamedIndividual rdf:about="http://purl.obolibrary.org/obo/GAZ_00123693">
        <obo:RO_0001025 rdf:resource="http://purl.obolibrary.org/obo/GAZ_00031139"/>
        <obo:IAO_0000115>One of the 77 woredas in the Southern Nations, Nationalities and Peoples&apos; Region of Ethiopia. Part of the Sidama Zone that extends into the Oromia Region like a peninsula, Bensa is bordered on the southeast and north by the Oromia Region, with Hula on the west and Arbegona on the northwest, and Aroresa on the east. The major town in Bensa is Daye.</obo:IAO_0000115>
        <oboInOwl:hasOBONamespace>GAZ</oboInOwl:hasOBONamespace>
        <oboInOwl:id>GAZ:00123693</oboInOwl:id>
        <rdfs:label>Bensa Woreda</rdfs:label>
    </owl:NamedIndividual>
    


    <!-- http://purl.obolibrary.org/obo/GAZ_00123694 -->

    <owl:NamedIndividual rdf:about="http://purl.obolibrary.org/obo/GAZ_00123694">
        <obo:RO_0001025 rdf:resource="http://purl.obolibrary.org/obo/GAZ_00031152"/>
        <obo:IAO_0000115>One of the 36 woredas in the Tigray Region of Ethiopia. Part of the Mi&apos;irabawi Zone, Kafta Humera is bordered on the south by Tsegede, on the west by Sudan, then by the Tekeze River which separates Kafta Humera from Eritrea on the north and Tahtay Adiyabo on the east, and on the southeast by Wolqayt. Its administrative center is Humera ; other towns in Kafta Humera include Addi Hirdi.</obo:IAO_0000115>
        <oboInOwl:hasOBONamespace>GAZ</oboInOwl:hasOBONamespace>
        <oboInOwl:id>GAZ:00123694</oboInOwl:id>
        <rdfs:label>Kafta Humera Woreda</rdfs:label>
    </owl:NamedIndividual>
    


    <!-- http://purl.obolibrary.org/obo/GAZ_00123695 -->

    <owl:NamedIndividual rdf:about="http://purl.obolibrary.org/obo/GAZ_00123695">
        <obo:RO_0001025 rdf:resource="http://purl.obolibrary.org/obo/GAZ_00031152"/>
        <obo:IAO_0000115>One of the 36 woredas in the Tigray Region of Ethiopia. Part of the Mi&apos;irabawi Zone, Tselemti is bordered on the south by the Amhara Region, on the west by Wolqayt, on the north by Asigede Tsimbela, and on the northeast from Medebay Zana, and on the east by the Mehakelegnaw (Central Area) Zone. The Tekeze defines the boundary between Tselemti and both the last two woredas and the Zone; other rivers in this woreda include the Abata, a tributary of the Tekeze. Towns in Tselemti include Dima and Maytsebri.</obo:IAO_0000115>
        <oboInOwl:hasOBONamespace>GAZ</oboInOwl:hasOBONamespace>
        <oboInOwl:id>GAZ:00123695</oboInOwl:id>
        <rdfs:label>Tselemti Woreda</rdfs:label>
    </owl:NamedIndividual>
    


    <!-- http://purl.obolibrary.org/obo/GAZ_00123696 -->

    <owl:NamedIndividual rdf:about="http://purl.obolibrary.org/obo/GAZ_00123696">
        <obo:RO_0001025 rdf:resource="http://purl.obolibrary.org/obo/GAZ_00031152"/>
        <obo:IAO_0000115>A woreda in northwestern Ethiopia. Located in Mi&apos;irabawi Zone in Tigray Region, this woreda is bordered on the northwest and north by Kafta Humera, then separated on the northeast by Tahtay Adiyabo and on the east by Asigede Tsimbela by the Tekeze River, on the southeast by Tselemti, and on the south by Tsegede. The administrative center of Wolqayt is Addi Remets; other towns in this woreda include Maygaba and Awura.</obo:IAO_0000115>
        <oboInOwl:hasOBONamespace>GAZ</oboInOwl:hasOBONamespace>
        <oboInOwl:id>GAZ:00123696</oboInOwl:id>
        <rdfs:label>Wolqayt Woreda</rdfs:label>
    </owl:NamedIndividual>
    


    <!-- http://purl.obolibrary.org/obo/GAZ_00123697 -->

    <owl:NamedIndividual rdf:about="http://purl.obolibrary.org/obo/GAZ_00123697">
        <obo:RO_0001025 rdf:resource="http://purl.obolibrary.org/obo/GAZ_00031152"/>
        <obo:IAO_0000115>One of the 36 woredas in the Tigray Region of Ethiopia. Part of the Mi&apos;irabawi Zone, Tahtay Adiyabo is bordered on the south by the Asigede Tsimbela, then by the Tekeze River which separates Tahtay Adiyabo from Wolqayt and Kafta Humera on the southwest, on the north by Eritrea, and on the east by La&apos;ilay Adiyabo. The administrative center of Tahtay Adiyabo is Shiraro; other towns in this woreda include Addi Awuala, Addi Hageray, and Badme.</obo:IAO_0000115>
        <oboInOwl:hasOBONamespace>GAZ</oboInOwl:hasOBONamespace>
        <oboInOwl:id>GAZ:00123697</oboInOwl:id>
        <rdfs:label>Tahtay Adiyabo Woreda</rdfs:label>
    </owl:NamedIndividual>
    


    <!-- http://purl.obolibrary.org/obo/GAZ_00123698 -->

    <owl:NamedIndividual rdf:about="http://purl.obolibrary.org/obo/GAZ_00123698">
        <obo:RO_0001025 rdf:resource="http://purl.obolibrary.org/obo/GAZ_00031152"/>
        <obo:IAO_0000115>One of the 36 woredas in the Tigray Region of Ethiopia. Part of the Mi&apos;irabawi Zone, Tahtay Koraro is bordered on the southwest by Asigede Tsimbela, on the north by La&apos;ilay Adiyabo, and on the southeast by Medebay Zana. Towns and cities in Tahtay Koraro include Inda Selassie and Semema.</obo:IAO_0000115>
        <oboInOwl:hasOBONamespace>GAZ</oboInOwl:hasOBONamespace>
        <oboInOwl:id>GAZ:00123698</oboInOwl:id>
        <rdfs:label>Tahtay Koraro Woreda</rdfs:label>
    </owl:NamedIndividual>
    


    <!-- http://purl.obolibrary.org/obo/GAZ_00123699 -->

    <owl:NamedIndividual rdf:about="http://purl.obolibrary.org/obo/GAZ_00123699">
        <obo:RO_0001025 rdf:resource="http://purl.obolibrary.org/obo/GAZ_00031152"/>
        <obo:IAO_0000115>One of the 36 woredas in the Tigray Region of Ethiopia. Part of the Mi&apos;irabawi Zone, La&apos;ilay Adiyabo is bordered on the south by Tahtay Koraro, on the southwest by Asigede Tsimbela, on the northwest by Tahtay Adiyabo, on the northeast by Eritrea, on the east by the Mehakelegnaw (Central) Zone, and on the southeast by Medebay Zana. Towns and cities in La&apos;ilay Adiyabo include Addi Daero and Addi Nebreid.</obo:IAO_0000115>
        <oboInOwl:hasOBONamespace>GAZ</oboInOwl:hasOBONamespace>
        <oboInOwl:id>GAZ:00123699</oboInOwl:id>
        <rdfs:label>La&apos;ilay Adiyabo Woreda</rdfs:label>
    </owl:NamedIndividual>
    


    <!-- http://purl.obolibrary.org/obo/GAZ_00123700 -->

    <owl:NamedIndividual rdf:about="http://purl.obolibrary.org/obo/GAZ_00123700">
        <obo:RO_0001025 rdf:resource="http://purl.obolibrary.org/obo/GAZ_00031152"/>
        <obo:IAO_0000115>Oe of the 36 woredas in the Tigray Region of Ethiopia. Part of the Mi&apos;irabawi Zone, Asegede Tsimbela is bordered along the south by the Tekeze River which separates the woreda on the south from Tselemti and to the west by Wolqayt, then on the northwest by La&apos;ilay Adiyabo, on the northeast by Tahtay Koraro, and on the east by Medebay Zana. Towns and cities in Asegede Tsimbela include Enda Aba Guna and Kisadgaba.</obo:IAO_0000115>
        <oboInOwl:hasOBONamespace>GAZ</oboInOwl:hasOBONamespace>
        <oboInOwl:id>GAZ:00123700</oboInOwl:id>
        <rdfs:label>Asigede Tsimbela Woreda</rdfs:label>
    </owl:NamedIndividual>
    


    <!-- http://purl.obolibrary.org/obo/GAZ_00123701 -->

    <owl:NamedIndividual rdf:about="http://purl.obolibrary.org/obo/GAZ_00123701">
        <obo:RO_0001025 rdf:resource="http://purl.obolibrary.org/obo/GAZ_00031152"/>
        <obo:IAO_0000115>One of the 36 woredas in the Tigray Region of Ethiopia. Part of the Mi&apos;irabawi Zone, Medebay Zana is bordered on the south by the Tekeze River which separates Tahtay Adiyabo from Tselemti, on the southwest by Asigede Tsimbela, on the northwest by Tahtay Koraro, on the north by La&apos;ilay Adiyabo, and on the east by the Mehakelegnaw (Central) Zone. Towns and cities in Medebay Zana include Debre Kerbe and Seleh Leha.</obo:IAO_0000115>
        <oboInOwl:hasOBONamespace>GAZ</oboInOwl:hasOBONamespace>
        <oboInOwl:id>GAZ:00123701</oboInOwl:id>
        <rdfs:label>Medebay Zana Woreda</rdfs:label>
    </owl:NamedIndividual>
    


    <!-- http://purl.obolibrary.org/obo/GAZ_00123702 -->

    <owl:NamedIndividual rdf:about="http://purl.obolibrary.org/obo/GAZ_00123702">
        <obo:RO_0001025 rdf:resource="http://purl.obolibrary.org/obo/GAZ_00031152"/>
        <obo:IAO_0000115>One of the 36 woredas in the Tigray Region of Ethiopia. It is named after the historic province of Tsegede. Part of the Mi&apos;irabawi Zone, Tsegede is bordered on the south and west by the Amhara Region, on the northwest by Kafta Humera, and on the north by Wolqayt. Towns in Tsegede include Idaga Hamus.</obo:IAO_0000115>
        <oboInOwl:hasOBONamespace>GAZ</oboInOwl:hasOBONamespace>
        <oboInOwl:id>GAZ:00123702</oboInOwl:id>
        <rdfs:label>Tsegede Woreda</rdfs:label>
    </owl:NamedIndividual>
    


    <!-- http://purl.obolibrary.org/obo/GAZ_00123703 -->

    <owl:NamedIndividual rdf:about="http://purl.obolibrary.org/obo/GAZ_00123703">
        <obo:RO_0001025 rdf:resource="http://purl.obolibrary.org/obo/GAZ_00031151"/>
        <obo:IAO_0000115>One of the 36 woredas in the Tigray Region of Ethiopia. Located in the Misraqawi Zone at the eastern edge of the Ethiopian highlands, Atsbi Wenberta is bordered on the south by the Debubawi (Southern) Zone, on the southwest by Wukro, and on the northwest by Saesi Tsaedaemba. Towns in Atsbi Wenberta include Atsbi and Haik Mesahil.</obo:IAO_0000115>
        <oboInOwl:hasOBONamespace>GAZ</oboInOwl:hasOBONamespace>
        <oboInOwl:id>GAZ:00123703</oboInOwl:id>
        <rdfs:label>Atsbi Wenberta Woreda</rdfs:label>
    </owl:NamedIndividual>
    


    <!-- http://purl.obolibrary.org/obo/GAZ_00123704 -->

    <owl:NamedIndividual rdf:about="http://purl.obolibrary.org/obo/GAZ_00123704">
        <obo:RO_0001025 rdf:resource="http://purl.obolibrary.org/obo/GAZ_00031151"/>
        <obo:IAO_0000115>One of the 36 woredas in the Tigray Region of Ethiopia. Located in the Misraqawi Zone at the eastern edge of the Ethiopian highlands, Saesi Tsaedaemba is bordered on the south by Wukro, on the southwest by Hawzen, on the west by Ganta Afeshum, on the northwest by Gulomahda, on the north by Irob, on the east by the Afar Region, and on the southeast by Atsbi Wenberta. Towns in Saesi Tsaedaemba include Edaga Hamus and Freweyni.</obo:IAO_0000115>
        <oboInOwl:hasOBONamespace>GAZ</oboInOwl:hasOBONamespace>
        <oboInOwl:id>GAZ:00123704</oboInOwl:id>
        <rdfs:label>Saesi Tsaedaemba Woreda</rdfs:label>
    </owl:NamedIndividual>
    


    <!-- http://purl.obolibrary.org/obo/GAZ_00123705 -->

    <owl:NamedIndividual rdf:about="http://purl.obolibrary.org/obo/GAZ_00123705">
        <obo:RO_0001025 rdf:resource="http://purl.obolibrary.org/obo/GAZ_00031151"/>
        <obo:IAO_0000115>One of the 36 woredas in the Tigray Region of Ethiopia. Part of the Misraqawi Zone, Ganta Afeshum is bordered on the south by Hawzen, on the west by the Mehakelegnaw (Central) Zone, on the north by Gulomahda, and on the east by Saesi Tsaedaemba. Towns in Ganta Afeshum include Adigrat and Bizet.</obo:IAO_0000115>
        <oboInOwl:hasOBONamespace>GAZ</oboInOwl:hasOBONamespace>
        <oboInOwl:id>GAZ:00123705</oboInOwl:id>
        <rdfs:label>Ganta Afeshum Woreda</rdfs:label>
    </owl:NamedIndividual>
    


    <!-- http://purl.obolibrary.org/obo/GAZ_00123706 -->

    <owl:NamedIndividual rdf:about="http://purl.obolibrary.org/obo/GAZ_00123706">
        <obo:RO_0001025 rdf:resource="http://purl.obolibrary.org/obo/GAZ_00031151"/>
        <obo:IAO_0000115>One of the 36 woredas in the Tigray Region of Ethiopia. Part of the Misraqawi Zone, Gulomakeda is bordered on the south by Ganta Afeshum, on the west by the Mehakelegnaw (Central) Zone, on the north by Eritrea, and on the east by Irob. Towns in Gulomakeda include Sebeya and Zalambessa.</obo:IAO_0000115>
        <oboInOwl:hasOBONamespace>GAZ</oboInOwl:hasOBONamespace>
        <oboInOwl:id>GAZ:00123706</oboInOwl:id>
        <rdfs:label>Gulomahda Woreda</rdfs:label>
    </owl:NamedIndividual>
    


    <!-- http://purl.obolibrary.org/obo/GAZ_00123707 -->

    <owl:NamedIndividual rdf:about="http://purl.obolibrary.org/obo/GAZ_00123707">
        <obo:RO_0001025 rdf:resource="http://purl.obolibrary.org/obo/GAZ_00031151"/>
        <obo:IAO_0000115>One of the 36 woredas in the Tigray Region of Ethiopia. Part of the Misraqawi Zone, Hawzen is bordered on the south by Wukro, on the west by the Mehakelegnaw (Central) Zone, on the north by Ganta Afeshum, and on the east by Saesi Tsaedaemba. Towns in Hawzen include Hawzen and Megab.</obo:IAO_0000115>
        <oboInOwl:hasOBONamespace>GAZ</oboInOwl:hasOBONamespace>
        <oboInOwl:id>GAZ:00123707</oboInOwl:id>
        <rdfs:label>Hawzen Woreda</rdfs:label>
    </owl:NamedIndividual>
    


    <!-- http://purl.obolibrary.org/obo/GAZ_00123708 -->

    <owl:NamedIndividual rdf:about="http://purl.obolibrary.org/obo/GAZ_00123708">
        <obo:RO_0001025 rdf:resource="http://purl.obolibrary.org/obo/GAZ_00031151"/>
        <obo:IAO_0000115>One of the 36 woredas in the Tigray Region of Ethiopia. This woreda is named after the Irob people, who are the predominant ethnic group living there. Located in the Misraqawi Zone at the eastern escarpment of the Ethiopian highlands, Irob is bordered on the south by Saesi Tsaedaemba, on the west by Gulomahda, on the north and east by Eritrea, and on the southeast by the Afar Region. The administrative center for this woreda is Alitena.</obo:IAO_0000115>
        <oboInOwl:hasOBONamespace>GAZ</oboInOwl:hasOBONamespace>
        <oboInOwl:id>GAZ:00123708</oboInOwl:id>
        <rdfs:label>Irob Woreda</rdfs:label>
    </owl:NamedIndividual>
    


    <!-- http://purl.obolibrary.org/obo/GAZ_00123709 -->

    <owl:NamedIndividual rdf:about="http://purl.obolibrary.org/obo/GAZ_00123709">
        <obo:RO_0001025 rdf:resource="http://purl.obolibrary.org/obo/GAZ_00031148"/>
        <obo:IAO_0000115>One of the 36 woredas in the Tigray Region of Ethiopia. Part of the Mehakelegnaw Zone, Naeder Adet is bordered on the south by Kola Tembien, on the west by Mi&apos;irabawi (Western) Zone, on the northwest by Tahtay Maychew, on the northeast by La&apos;ilay Maychew, and on the east by Werie Lehe. Towns in Naeder Adet include Edaga Selus.</obo:IAO_0000115>
        <oboInOwl:hasOBONamespace>GAZ</oboInOwl:hasOBONamespace>
        <oboInOwl:id>GAZ:00123709</oboInOwl:id>
        <rdfs:label>Naeder Adet Woreda</rdfs:label>
    </owl:NamedIndividual>
    


    <!-- http://purl.obolibrary.org/obo/GAZ_00123710 -->

    <owl:NamedIndividual rdf:about="http://purl.obolibrary.org/obo/GAZ_00123710">
        <obo:RO_0001025 rdf:resource="http://purl.obolibrary.org/obo/GAZ_00031148"/>
        <obo:IAO_0000115>One of the 36 woredas in the Tigray Region of Ethiopia. Part of the Mehakelegnaw Zone, Mereb Lehe is bordered on the south by La&apos;ilay Maychew, on the southwest by Tahtay Maychew, on the west by the Mi&apos;irabawi (Western) Zone, on the north by Eritrea, on the east by Enticho, and on the southeast by Adwa. The administrative center of this woreda is Rama; other towns include La&apos;ilay Merhisenay.</obo:IAO_0000115>
        <oboInOwl:hasOBONamespace>GAZ</oboInOwl:hasOBONamespace>
        <oboInOwl:id>GAZ:00123710</oboInOwl:id>
        <rdfs:label>Mereb Lehe Woreda</rdfs:label>
    </owl:NamedIndividual>
    


    <!-- http://purl.obolibrary.org/obo/GAZ_00123711 -->

    <owl:NamedIndividual rdf:about="http://purl.obolibrary.org/obo/GAZ_00123711">
        <obo:RO_0001025 rdf:resource="http://purl.obolibrary.org/obo/GAZ_00031148"/>
        <obo:IAO_0000115>One of the 36 woredas in the Tigray Region of Ethiopia. It is named in part after the former province of Tembien. Part of the Mehakelegnaw Zone, Kola Tembien is bordered on the south by Abergele, then by the Tekeze River on the west which separates it on the west from the Mi&apos;irabawi (Western) Zone, on the northwest by Naeder Adet, on the northeast by Werie Lehe, and on the east by Misraqawi (Eastern) Zone. Towns in Kola Tembien include Abiy Addi, Guya and Werkamba.</obo:IAO_0000115>
        <oboInOwl:hasOBONamespace>GAZ</oboInOwl:hasOBONamespace>
        <oboInOwl:id>GAZ:00123711</oboInOwl:id>
        <rdfs:label>Kola Tembien Woreda</rdfs:label>
    </owl:NamedIndividual>
    


    <!-- http://purl.obolibrary.org/obo/GAZ_00123712 -->

    <owl:NamedIndividual rdf:about="http://purl.obolibrary.org/obo/GAZ_00123712">
        <obo:RO_0001025 rdf:resource="http://purl.obolibrary.org/obo/GAZ_00031148"/>
        <obo:IAO_0000115>One of the 36 woredas in the Tigray Region of Ethiopia. Part of the Mehakelegnaw Zone, Tahtay Maychew is bordered on the south by Naeder Adet, on the west by the Mi&apos;irabawi (Western) Zone, on the north by Mereb Lehe, and on the east by La&apos;alay Maychew. Towns in Tahtay Maychew include Chila and Wukro Maray.</obo:IAO_0000115>
        <oboInOwl:hasOBONamespace>GAZ</oboInOwl:hasOBONamespace>
        <oboInOwl:id>GAZ:00123712</oboInOwl:id>
        <rdfs:label>Tahtay Maychew Woreda</rdfs:label>
    </owl:NamedIndividual>
    


    <!-- http://purl.obolibrary.org/obo/GAZ_00123713 -->

    <owl:NamedIndividual rdf:about="http://purl.obolibrary.org/obo/GAZ_00123713">
        <obo:RO_0001025 rdf:resource="http://purl.obolibrary.org/obo/GAZ_00031148"/>
        <obo:IAO_0000115>One of the 36 woredas in the Tigray Region of Ethiopia. It is named in part after the former province of Tembien. Part of the Mehakelegnaw Zone, Degua Tembien is bordered on the south by the Debubawi (South) Zone, on the west by Abergele, on the north by Kola Tembien, and on the east by the Misraqawi (Eastern) Zone. Towns in Degua Tembien include Hagera Selam.</obo:IAO_0000115>
        <oboInOwl:hasOBONamespace>GAZ</oboInOwl:hasOBONamespace>
        <oboInOwl:id>GAZ:00123713</oboInOwl:id>
        <rdfs:label>Degua Tembien Woreda</rdfs:label>
    </owl:NamedIndividual>
    


    <!-- http://purl.obolibrary.org/obo/GAZ_00123714 -->

    <owl:NamedIndividual rdf:about="http://purl.obolibrary.org/obo/GAZ_00123714">
        <obo:RO_0001025 rdf:resource="http://purl.obolibrary.org/obo/GAZ_00031148"/>
        <obo:IAO_0000115>One of the 36 woredas in the Tigray Region of Ethiopia. Part of the Mehakelegnaw Zone, Abergele is bordered on the south and west by the Amhara Region, then by the Tekeze River on the west, on the north by Kola Tembien, on the east by Degua Tembien and on the southeast by the Debubawi (Southern) Zone. Towns in Abergele include Agbe and Yechila.</obo:IAO_0000115>
        <oboInOwl:hasOBONamespace>GAZ</oboInOwl:hasOBONamespace>
        <oboInOwl:id>GAZ:00123714</oboInOwl:id>
        <rdfs:label>Abergele Woreda</rdfs:label>
    </owl:NamedIndividual>
    


    <!-- http://purl.obolibrary.org/obo/GAZ_00123715 -->

    <owl:NamedIndividual rdf:about="http://purl.obolibrary.org/obo/GAZ_00123715">
        <obo:RO_0001025 rdf:resource="http://purl.obolibrary.org/obo/GAZ_00031148"/>
        <obo:IAO_0000115>One of the 36 woredas in the Tigray Region of Ethiopia. Part of the Mehakelegnaw Zone, Enticho is bordered on the south by Werie Lehe, on the southwest by Adwa, on the west by Mereb Lehe, on the north by Eritrea, and on the east by the Misraqawi (Eastern) Zone. Towns in Enticho include Edaga Arbi, Enticho and Gerhusernay.</obo:IAO_0000115>
        <oboInOwl:hasOBONamespace>GAZ</oboInOwl:hasOBONamespace>
        <oboInOwl:id>GAZ:00123715</oboInOwl:id>
        <rdfs:label>Enticho Woreda</rdfs:label>
    </owl:NamedIndividual>
    


    <!-- http://purl.obolibrary.org/obo/GAZ_00123716 -->

    <owl:NamedIndividual rdf:about="http://purl.obolibrary.org/obo/GAZ_00123716">
        <obo:RO_0001025 rdf:resource="http://purl.obolibrary.org/obo/GAZ_00031148"/>
        <obo:IAO_0000115>One of the 36 woredas in the Tigray Region of Ethiopia. Part of the Mehakelegnaw Zone, La&apos;ilay Maychew is bordered on the south by Naeder Adet, on the west by Tahtay Maychew, on the north by Mereb Lehe, and on the east by Adwa. Towns in La&apos;ilay Maychew include Axum and Mahibere Degue.</obo:IAO_0000115>
        <oboInOwl:hasOBONamespace>GAZ</oboInOwl:hasOBONamespace>
        <oboInOwl:id>GAZ:00123716</oboInOwl:id>
        <rdfs:label>La&apos;ilay Maychew Woreda</rdfs:label>
    </owl:NamedIndividual>
    


    <!-- http://purl.obolibrary.org/obo/GAZ_00123717 -->

    <owl:NamedIndividual rdf:about="http://purl.obolibrary.org/obo/GAZ_00123717">
        <obo:RO_0001025 rdf:resource="http://purl.obolibrary.org/obo/GAZ_00031148"/>
        <obo:IAO_0000115>One of the 36 woredas in the Tigray Region of Ethiopia. Part of the Mehakelegnaw Zone, Adwa is bordered on the south by Werie Lehe, on the west by La&apos;ilay Maychew, on the north by Mereb Lehe, and on the east by Enticho. The major town in this woreda is Adwa.</obo:IAO_0000115>
        <oboInOwl:hasOBONamespace>GAZ</oboInOwl:hasOBONamespace>
        <oboInOwl:id>GAZ:00123717</oboInOwl:id>
        <rdfs:label>Adwa Woreda</rdfs:label>
    </owl:NamedIndividual>
    


    <!-- http://purl.obolibrary.org/obo/GAZ_00123718 -->

    <owl:NamedIndividual rdf:about="http://purl.obolibrary.org/obo/GAZ_00123718">
        <obo:RO_0001025 rdf:resource="http://purl.obolibrary.org/obo/GAZ_00031148"/>
        <obo:IAO_0000115>One of the 36 woredas in the Tigray Region of Ethiopia. Part of the Mehakelegnaw Zone, Werie Lehe is bordered on the south by Kola Tembien, on the southwest by Naeder Adet, on the west by La&apos;ilay Maychew, on the north by Adwa, on the northeast by Enticho, and on the east by the Misraqawi (Eastern) Zone. Towns in Werie Lehe include Edaga Arbi, Maykinetal, and Nebelet.</obo:IAO_0000115>
        <oboInOwl:hasOBONamespace>GAZ</oboInOwl:hasOBONamespace>
        <oboInOwl:id>GAZ:00123718</oboInOwl:id>
        <rdfs:label>Werie Lehe Woreda</rdfs:label>
    </owl:NamedIndividual>
    


    <!-- http://purl.obolibrary.org/obo/GAZ_00123719 -->

    <owl:NamedIndividual rdf:about="http://purl.obolibrary.org/obo/GAZ_00123719">
        <obo:RO_0001025 rdf:resource="http://purl.obolibrary.org/obo/GAZ_00031149"/>
        <obo:IAO_0000115>One of the 36 woredas in the Tigray Region of Ethiopia. Part of the Debubawi Zone, Alaje is bordered on the south by Endamehoni, on the west by the Amhara Region, on the northwest by Samre, on the northeast by Hintalo Wajirat, and on the east by Raya Azebo. Towns in Alaje include Adi Shenu, Chelena and Dela.</obo:IAO_0000115>
        <oboInOwl:hasOBONamespace>GAZ</oboInOwl:hasOBONamespace>
        <oboInOwl:id>GAZ:00123719</oboInOwl:id>
        <rdfs:label>Alaje Woreda</rdfs:label>
    </owl:NamedIndividual>
    


    <!-- http://purl.obolibrary.org/obo/GAZ_00123720 -->

    <owl:NamedIndividual rdf:about="http://purl.obolibrary.org/obo/GAZ_00123720">
        <obo:RO_0001025 rdf:resource="http://purl.obolibrary.org/obo/GAZ_00031149"/>
        <obo:IAO_0000115>One of the 36 woredas in the Tigray Region of Ethiopia. Part of the Debubawi Zone, Ofla is bordered on the south by Alamata, on the west by the Amhara Region, on the north by Endamehoni, and on the east by Raya Azebo.</obo:IAO_0000115>
        <oboInOwl:hasOBONamespace>GAZ</oboInOwl:hasOBONamespace>
        <oboInOwl:id>GAZ:00123720</oboInOwl:id>
        <rdfs:label>Ofla Woreda</rdfs:label>
    </owl:NamedIndividual>
    


    <!-- http://purl.obolibrary.org/obo/GAZ_00123721 -->

    <owl:NamedIndividual rdf:about="http://purl.obolibrary.org/obo/GAZ_00123721">
        <obo:RO_0001025 rdf:resource="http://purl.obolibrary.org/obo/GAZ_00031149"/>
        <obo:IAO_0000115>One of the 36 woredas in the Tigray Region of Ethiopia. Part of the Debubawi Zone, Samre is bordered on the south by the Amhara Region, on the west and north by the Mehakelegnaw (Central) Zone, on the northeast by Enderta, on the east by Hintalo Wajirat, and on the southeast by Alaje. Towns in Samre include Gijet and Samre.</obo:IAO_0000115>
        <oboInOwl:hasOBONamespace>GAZ</oboInOwl:hasOBONamespace>
        <oboInOwl:id>GAZ:00123721</oboInOwl:id>
        <rdfs:label>Samre Woreda</rdfs:label>
    </owl:NamedIndividual>
    


    <!-- http://purl.obolibrary.org/obo/GAZ_00123722 -->

    <owl:NamedIndividual rdf:about="http://purl.obolibrary.org/obo/GAZ_00123722">
        <obo:RO_0001025 rdf:resource="http://purl.obolibrary.org/obo/GAZ_00031149"/>
        <obo:IAO_0000115>One of the 36 woredas in the Tigray Region of Ethiopia. Part of the Debubawi Zone, Alamata is bordered on the south and west by the Amhara Region, on the northwest by Ofla, and on the northeast by Raya Azebo. The administrative center is Alamata; other towns in Alamata include Waja.</obo:IAO_0000115>
        <oboInOwl:hasOBONamespace>GAZ</oboInOwl:hasOBONamespace>
        <oboInOwl:id>GAZ:00123722</oboInOwl:id>
        <rdfs:label>Alamata Woreda</rdfs:label>
    </owl:NamedIndividual>
    


    <!-- http://purl.obolibrary.org/obo/GAZ_00123724 -->

    <owl:NamedIndividual rdf:about="http://purl.obolibrary.org/obo/GAZ_00123724">
        <obo:RO_0001025 rdf:resource="http://purl.obolibrary.org/obo/GAZ_00031149"/>
        <obo:IAO_0000115>One of the 36 woredas in the Tigray Region of Ethiopia. Located in the Debubawi Zone at the eastern edge of the Ethiopian highlands, Debubawi Zone, Enderta is bordered on the south by Hintalo Wajirat, on the west by Samre, on the northwest and north by the Misraqawi (Eastern) Zone, and on the east by the Afar Region; the city and woreda of Mek&apos;ele is an enclave within Enderta. Towns in Enderta include Aynalem and Qwiha.</obo:IAO_0000115>
        <oboInOwl:hasOBONamespace>GAZ</oboInOwl:hasOBONamespace>
        <oboInOwl:id>GAZ:00123724</oboInOwl:id>
        <rdfs:label>Enderta Woreda</rdfs:label>
    </owl:NamedIndividual>
    


    <!-- http://purl.obolibrary.org/obo/GAZ_00123725 -->

    <owl:NamedIndividual rdf:about="http://purl.obolibrary.org/obo/GAZ_00123725">
        <obo:RO_0001025 rdf:resource="http://purl.obolibrary.org/obo/GAZ_00031149"/>
        <obo:IAO_0000115>One of the 36 woredas in the Tigray Region of Ethiopia. Located in the Debubawi Zone at the eastern edge of the Ethiopian highlands, Debubawi Zone, Raya Azebo is bordered on the south by Alamata, on the southwest by Ofla, on the northwest by Endamehoni, on the north by Hintalo Wajirat, and on the east by the Afar Region. Towns in Raya Azebo include Mersa and Weyra Wuha.</obo:IAO_0000115>
        <oboInOwl:hasOBONamespace>GAZ</oboInOwl:hasOBONamespace>
        <oboInOwl:id>GAZ:00123725</oboInOwl:id>
        <rdfs:label>Raya Azebo Woreda</rdfs:label>
    </owl:NamedIndividual>
    


    <!-- http://purl.obolibrary.org/obo/GAZ_00123726 -->

    <owl:NamedIndividual rdf:about="http://purl.obolibrary.org/obo/GAZ_00123726">
        <obo:RO_0001025 rdf:resource="http://purl.obolibrary.org/obo/GAZ_00031149"/>
        <obo:IAO_0000115>One of the 36 woredas in the Tigray Region of Ethiopia. Located in the Debubawi Zone at the eastern edge of the Ethiopian highlands, Debubawi Zone, Hintalo Wajirat is bordered on the south by Raya Azebo, on the southwest by Alaje, on the west by Samre, on the north by Enderta, and on the east by the Afar Region; Hintalo Wajirat surrounds the woreda of Mek&apos;ele on all sides.</obo:IAO_0000115>
        <oboInOwl:hasOBONamespace>GAZ</oboInOwl:hasOBONamespace>
        <oboInOwl:id>GAZ:00123726</oboInOwl:id>
        <rdfs:label>Hintalo Wajirat Woreda</rdfs:label>
    </owl:NamedIndividual>
    


    <!-- http://purl.obolibrary.org/obo/GAZ_00123727 -->

    <owl:NamedIndividual rdf:about="http://purl.obolibrary.org/obo/GAZ_00123727">
        <obo:RO_0001025 rdf:resource="http://purl.obolibrary.org/obo/GAZ_00031149"/>
        <obo:IAO_0000115>One of the 36 woredas in the Tigray Region of Ethiopia. Part of the Debubawi Zone, Endamehoni is bordered on the south by Ofla, on the west by the Amhara Region, on the north by Alaje, and on the east by Raya Azebo. The administrative center of Endamehoni is Maychew; other towns include Wedisemro.</obo:IAO_0000115>
        <oboInOwl:hasOBONamespace>GAZ</oboInOwl:hasOBONamespace>
        <oboInOwl:id>GAZ:00123727</oboInOwl:id>
        <rdfs:label>Endamehoni Woreda</rdfs:label>
    </owl:NamedIndividual>
    


    <!-- http://purl.obolibrary.org/obo/GAZ_00123734 -->

    <owl:NamedIndividual rdf:about="http://purl.obolibrary.org/obo/GAZ_00123734">
        <obo:RO_0001025 rdf:resource="http://purl.obolibrary.org/obo/GAZ_00031117"/>
        <obo:IAO_0000115>One of the 180 woredas in the Oromia Region of Ethiopia. Part of the Arsi Zone.</obo:IAO_0000115>
        <oboInOwl:hasOBONamespace>GAZ</oboInOwl:hasOBONamespace>
        <oboInOwl:id>GAZ:00123734</oboInOwl:id>
        <rdfs:label>Digelu Tijo Woreda</rdfs:label>
    </owl:NamedIndividual>
    


    <!-- http://purl.obolibrary.org/obo/GAZ_00123735 -->

    <owl:NamedIndividual rdf:about="http://purl.obolibrary.org/obo/GAZ_00123735">
        <obo:RO_0001025 rdf:resource="http://purl.obolibrary.org/obo/GAZ_00031117"/>
        <obo:IAO_0000115>One of the 180 woredas in the Oromia Region of Ethiopia. Part of the Arsi Zone, Bekoji is bordered on the south by Gedeb, on the southwest by Kofele, on the west by Munesa, on the north by Digeluna Tijo, on the east by Sherka, and on the southeast by the Shebelle River which separates it from the Bale Zone. The administrative center of this woreda is Bekoji; other towns include Lemu Sirba, Meraro, Siltana and Sirbo.</obo:IAO_0000115>
        <oboInOwl:hasOBONamespace>GAZ</oboInOwl:hasOBONamespace>
        <oboInOwl:id>GAZ:00123735</oboInOwl:id>
        <rdfs:label>Bekoji Woreda</rdfs:label>
    </owl:NamedIndividual>
    


    <!-- http://purl.obolibrary.org/obo/GAZ_00123736 -->

    <owl:NamedIndividual rdf:about="http://purl.obolibrary.org/obo/GAZ_00123736">
        <obo:RO_0001025 rdf:resource="http://purl.obolibrary.org/obo/GAZ_00031117"/>
        <obo:IAO_0000115>One of the 180 woredas in the Oromia Region of Ethiopia. Part of the Arsi Zone located in the Great Rift Valley, Ziway Dugda is bordered on the south by Munesa, on the west and north by the Misraq Shewa Zone, on the east by Hitosa, and on the southeast by Tiyo. The woreda capital is Ogolcho.</obo:IAO_0000115>
        <oboInOwl:hasOBONamespace>GAZ</oboInOwl:hasOBONamespace>
        <oboInOwl:id>GAZ:00123736</oboInOwl:id>
        <rdfs:label>Ziway Dugda Woreda</rdfs:label>
    </owl:NamedIndividual>
    


    <!-- http://purl.obolibrary.org/obo/GAZ_00123737 -->

    <owl:NamedIndividual rdf:about="http://purl.obolibrary.org/obo/GAZ_00123737">
        <obo:RO_0001025 rdf:resource="http://purl.obolibrary.org/obo/GAZ_00031117"/>
        <obo:IAO_0000115>One of the 180 woredas in the Oromia Region of Ethiopia. Part of the Arsi Zone, Gololcha is bordered on the south by Amigna, on the west by Chole, on the northwest by Aseko, and on the north and east by the Mirab (West) Hararghe Zone. The woreda capital is Debre Selam (also known as Chencho); other towns include Timuga.</obo:IAO_0000115>
        <oboInOwl:hasOBONamespace>GAZ</oboInOwl:hasOBONamespace>
        <oboInOwl:id>GAZ:00123737</oboInOwl:id>
        <rdfs:label>Gololcha Woreda</rdfs:label>
    </owl:NamedIndividual>
    


    <!-- http://purl.obolibrary.org/obo/GAZ_00123738 -->

    <owl:NamedIndividual rdf:about="http://purl.obolibrary.org/obo/GAZ_00123738">
        <obo:RO_0001025 rdf:resource="http://purl.obolibrary.org/obo/GAZ_00031117"/>
        <obo:IAO_0000115>One of the 180 woredas in the Oromia Region of Ethiopia. Part of the Arsi Zone, Chole is bordered on the south by Amigna, on the southwest by Sude, on the northwest by Merti, on the north by Aseko, and on the east by Gololcha. Towns in Chole include Chole and Moye.</obo:IAO_0000115>
        <oboInOwl:hasOBONamespace>GAZ</oboInOwl:hasOBONamespace>
        <oboInOwl:id>GAZ:00123738</oboInOwl:id>
        <rdfs:label>Chole Woreda</rdfs:label>
    </owl:NamedIndividual>
    


    <!-- http://purl.obolibrary.org/obo/GAZ_00123739 -->

    <owl:NamedIndividual rdf:about="http://purl.obolibrary.org/obo/GAZ_00123739">
        <obo:RO_0001025 rdf:resource="http://purl.obolibrary.org/obo/GAZ_00031117"/>
        <obo:IAO_0000115>One of the 180 woredas in the Oromia Region of Ethiopia. Part of the Arsi Zone, Merti is bordered on the south by Sude, on the west by Jeju, on the northwest by the Misraq Shewa Zone, on the north by the Afar Region, on the east by Aseko, and on the southeast by Chole. The woreda capital is Abomsa; other towns include Reye.</obo:IAO_0000115>
        <oboInOwl:hasOBONamespace>GAZ</oboInOwl:hasOBONamespace>
        <oboInOwl:id>GAZ:00123739</oboInOwl:id>
        <rdfs:label>Merti Woreda</rdfs:label>
    </owl:NamedIndividual>
    


    <!-- http://purl.obolibrary.org/obo/GAZ_00123740 -->

    <owl:NamedIndividual rdf:about="http://purl.obolibrary.org/obo/GAZ_00123740">
        <obo:RO_0001025 rdf:resource="http://purl.obolibrary.org/obo/GAZ_00031117"/>
        <obo:IAO_0000115>One of the 180 woredas in the Oromia Region of Ethiopia. Part of the Arsi Zone, Aseko is bordered on the southwest by Chole, on the northwest by Merti, on the north by the Mirab (West) Hararghe Zone, and on the east by Gololcha.</obo:IAO_0000115>
        <oboInOwl:hasOBONamespace>GAZ</oboInOwl:hasOBONamespace>
        <oboInOwl:id>GAZ:00123740</oboInOwl:id>
        <rdfs:label>Aseko Woreda</rdfs:label>
    </owl:NamedIndividual>
    


    <!-- http://purl.obolibrary.org/obo/GAZ_00123741 -->

    <owl:NamedIndividual rdf:about="http://purl.obolibrary.org/obo/GAZ_00123741">
        <obo:RO_0001025 rdf:resource="http://purl.obolibrary.org/obo/GAZ_00031117"/>
        <obo:IAO_0000115>One of the 180 woredas in the Oromia Region of Ethiopia. Part of the Arsi Zone, Jeju is bordered by Dodotana Sire to the west, the Misraq Shewa Zone to the north, Merti to the east, and Sude to the south. Its administrative centre is Arboye, located 168 km southeast of Addis Ababa. Other towns in this woreda include Bolo.</obo:IAO_0000115>
        <oboInOwl:hasOBONamespace>GAZ</oboInOwl:hasOBONamespace>
        <oboInOwl:id>GAZ:00123741</oboInOwl:id>
        <rdfs:label>Jeju Woreda</rdfs:label>
    </owl:NamedIndividual>
    


    <!-- http://purl.obolibrary.org/obo/GAZ_00123742 -->

    <owl:NamedIndividual rdf:about="http://purl.obolibrary.org/obo/GAZ_00123742">
        <obo:RO_0001025 rdf:resource="http://purl.obolibrary.org/obo/GAZ_00031117"/>
        <obo:IAO_0000115>One of the 180 woredas in the Oromia Region of Ethiopia. Part of the Arsi Zone.</obo:IAO_0000115>
        <oboInOwl:hasOBONamespace>GAZ</oboInOwl:hasOBONamespace>
        <oboInOwl:id>GAZ:00123742</oboInOwl:id>
        <rdfs:label>Dodota Sire Woreda</rdfs:label>
    </owl:NamedIndividual>
    


    <!-- http://purl.obolibrary.org/obo/GAZ_00123743 -->

    <owl:NamedIndividual rdf:about="http://purl.obolibrary.org/obo/GAZ_00123743">
        <obo:RO_0001025 rdf:resource="http://purl.obolibrary.org/obo/GAZ_00031117"/>
        <obo:IAO_0000115>One of the 180 woredas in the Oromia Region of Ethiopia. Part of the Arsi Zone, Kofele is bordered on the south by the Bale Zone, on the southwest by the Southern Nations, Nationalities and Peoples&apos; Region, on the northwest by the Mirab Shewa Zone, on the north by Munesa, on the northeast by Bekoji, and on the east by Gedeb. Other towns in Kofele include Kore and Wabe Gefersa.</obo:IAO_0000115>
        <oboInOwl:hasOBONamespace>GAZ</oboInOwl:hasOBONamespace>
        <oboInOwl:id>GAZ:00123743</oboInOwl:id>
        <rdfs:label>Kofele Woreda</rdfs:label>
    </owl:NamedIndividual>
    


    <!-- http://purl.obolibrary.org/obo/GAZ_00123744 -->

    <owl:NamedIndividual rdf:about="http://purl.obolibrary.org/obo/GAZ_00123744">
        <obo:RO_0001025 rdf:resource="http://purl.obolibrary.org/obo/GAZ_00031117"/>
        <obo:IAO_0000115>One of the 180 woredas in the Oromia Region of Ethiopia. Part of the Arsi Zone, Amigna is bordered on the south by Seru, on the southwest by Robe, on the west by Sude, on the northwest by Chole, on the north by Gololcha, and on the east by the Mirab (West) Hararghe Zone. Towns include Adele.</obo:IAO_0000115>
        <oboInOwl:hasOBONamespace>GAZ</oboInOwl:hasOBONamespace>
        <oboInOwl:id>GAZ:00123744</oboInOwl:id>
        <rdfs:label>Amigna Woreda</rdfs:label>
    </owl:NamedIndividual>
    


    <!-- http://purl.obolibrary.org/obo/GAZ_00123745 -->

    <owl:NamedIndividual rdf:about="http://purl.obolibrary.org/obo/GAZ_00123745">
        <obo:RO_0001025 rdf:resource="http://purl.obolibrary.org/obo/GAZ_00031117"/>
        <obo:IAO_0000115>One of the 180 woredas in the Oromia Region of Ethiopia. Part of the Arsi Zone, Seru is bordered on the south and east by the Shebelle River which separates it from the Bale Zone, on the west by the Wabe River which separates it from Robe, on the north by Amigna, and on the northeast by the Mirab (West) Hararghe Zone. Other towns include Bele.</obo:IAO_0000115>
        <oboInOwl:hasOBONamespace>GAZ</oboInOwl:hasOBONamespace>
        <oboInOwl:id>GAZ:00123745</oboInOwl:id>
        <rdfs:label>Seru Woreda</rdfs:label>
    </owl:NamedIndividual>
    


    <!-- http://purl.obolibrary.org/obo/GAZ_00123746 -->

    <owl:NamedIndividual rdf:about="http://purl.obolibrary.org/obo/GAZ_00123746">
        <obo:RO_0001025 rdf:resource="http://purl.obolibrary.org/obo/GAZ_00031117"/>
        <obo:IAO_0000115>One of the 180 woredas in the Oromia Region of Ethiopia. Part of the Arsi Zone, Tiyo is bordered on the south by Munesa, on the west by Ziway Dugda, on the northeast by Hitosa, and on the southeast by Digeluna Tijo. The woreda and Zonal capital is Asella; other towns include Gonde.</obo:IAO_0000115>
        <oboInOwl:hasOBONamespace>GAZ</oboInOwl:hasOBONamespace>
        <oboInOwl:id>GAZ:00123746</oboInOwl:id>
        <rdfs:label>Tiyo Woreda</rdfs:label>
    </owl:NamedIndividual>
    


    <!-- http://purl.obolibrary.org/obo/GAZ_00123747 -->

    <owl:NamedIndividual rdf:about="http://purl.obolibrary.org/obo/GAZ_00123747">
        <obo:RO_0001025 rdf:resource="http://purl.obolibrary.org/obo/GAZ_00031117"/>
        <obo:IAO_0000115>One of the 180 woredas in the Oromia Region of Ethiopia. Part of the Arsi Zone located in the Great Rift Valley, Munesa is bordered on the south by Kofele, on the west by the Mirab Shewa Zone and Lake Langano, on the northwest by Ziway Dugda, on the north by Tiyo, on the northeast by Digeluna Tijo, and on the east by Bekoji. The woreda capital is Kersa; other towns include Ego.</obo:IAO_0000115>
        <oboInOwl:hasOBONamespace>GAZ</oboInOwl:hasOBONamespace>
        <oboInOwl:id>GAZ:00123747</oboInOwl:id>
        <rdfs:label>Munesa Woreda</rdfs:label>
    </owl:NamedIndividual>
    


    <!-- http://purl.obolibrary.org/obo/GAZ_00123748 -->

    <owl:NamedIndividual rdf:about="http://purl.obolibrary.org/obo/GAZ_00123748">
        <obo:RO_0001025 rdf:resource="http://purl.obolibrary.org/obo/GAZ_00031117"/>
        <obo:IAO_0000115>One of the 180 woredas in the Oromia Region of Ethiopia. Part of the Arsi Zone, Sude is bordered on the south by Robe, on the southwest by Tena,[1] on the west by Dodotana Sire, on the northwest by Jeju, on the north by Merti, on the northeast by Chole and on the southeast by Amigna. The woreda capital is Kula.</obo:IAO_0000115>
        <oboInOwl:hasOBONamespace>GAZ</oboInOwl:hasOBONamespace>
        <oboInOwl:id>GAZ:00123748</oboInOwl:id>
        <rdfs:label>Sude Woreda</rdfs:label>
    </owl:NamedIndividual>
    


    <!-- http://purl.obolibrary.org/obo/GAZ_00123749 -->

    <owl:NamedIndividual rdf:about="http://purl.obolibrary.org/obo/GAZ_00123749">
        <obo:RO_0001025 rdf:resource="http://purl.obolibrary.org/obo/GAZ_00031117"/>
        <obo:IAO_0000115>One of the 180 woredas in the Oromia Region of Ethiopia. Part of the Arsi Zone, Sherka is bordered on the south by the Shebelle River which separates it from the Bale Zone, on the southwest by Bekoji, on the west by Digeluna Tijo, on the north by Tena, and on the east by Robe. Gobesa is the administrative center; other towns include Gado Guna.</obo:IAO_0000115>
        <oboInOwl:hasOBONamespace>GAZ</oboInOwl:hasOBONamespace>
        <oboInOwl:id>GAZ:00123749</oboInOwl:id>
        <rdfs:label>Sherka Woreda</rdfs:label>
    </owl:NamedIndividual>
    


    <!-- http://purl.obolibrary.org/obo/GAZ_00123750 -->

    <owl:NamedIndividual rdf:about="http://purl.obolibrary.org/obo/GAZ_00123750">
        <obo:RO_0001025 rdf:resource="http://purl.obolibrary.org/obo/GAZ_00031117"/>
        <obo:IAO_0000115>One of the 180 woredas in the Oromia Region of Ethiopia. Part of the Arsi Zone, Hitosa is bordered on the south by Digeluna Tijo, on the southwest by Tiyo, on the west by Ziway Dugda, on the northwest by the Misraq Shewa Zone, on the northeast by Dodotana Sire, and on the east by Tena. The administrative center of the woreda is Iteya; other towns include Arb Gebeya, Borujawi, Huruta and Ligaba.</obo:IAO_0000115>
        <oboInOwl:hasOBONamespace>GAZ</oboInOwl:hasOBONamespace>
        <oboInOwl:id>GAZ:00123750</oboInOwl:id>
        <rdfs:label>Hitosa Woreda</rdfs:label>
    </owl:NamedIndividual>
    


    <!-- http://purl.obolibrary.org/obo/GAZ_00123751 -->

    <owl:NamedIndividual rdf:about="http://purl.obolibrary.org/obo/GAZ_00123751">
        <obo:RO_0001025 rdf:resource="http://purl.obolibrary.org/obo/GAZ_00031117"/>
        <obo:IAO_0000115>One of the 180 woredas in the Oromia Region of Ethiopia. Part of the Arsi Zone, Tena is bordered on the south by Sherka, on the southwest by Bekoji, on the west by Digeluna Tijo, on the northwest by Hitosa, on the north by Dodotana Sire, on the northeast by Sude, and on the east by Robe. The woreda capital is Ticho; other towns include Kela.</obo:IAO_0000115>
        <oboInOwl:hasOBONamespace>GAZ</oboInOwl:hasOBONamespace>
        <oboInOwl:id>GAZ:00123751</oboInOwl:id>
        <rdfs:label>Tena Woreda</rdfs:label>
    </owl:NamedIndividual>
    


    <!-- http://purl.obolibrary.org/obo/GAZ_00123752 -->

    <owl:NamedIndividual rdf:about="http://purl.obolibrary.org/obo/GAZ_00123752">
        <obo:RO_0001025 rdf:resource="http://purl.obolibrary.org/obo/GAZ_00031117"/>
        <obo:IAO_0000115>One of the 180 woredas in the Oromia Region of Ethiopia. Part of the Arsi Zone, Gedeb is bordered on the south by the Bale Zone, on the west by Kofele, and on the north and east by Bekoji. The woreda capital is Asasa.</obo:IAO_0000115>
        <oboInOwl:hasOBONamespace>GAZ</oboInOwl:hasOBONamespace>
        <oboInOwl:id>GAZ:00123752</oboInOwl:id>
        <rdfs:label>Gedeb Woreda</rdfs:label>
    </owl:NamedIndividual>
    


    <!-- http://purl.obolibrary.org/obo/GAZ_00123753 -->

    <owl:NamedIndividual rdf:about="http://purl.obolibrary.org/obo/GAZ_00123753">
        <obo:RO_0001025 rdf:resource="http://purl.obolibrary.org/obo/GAZ_00031117"/>
        <obo:IAO_0000115>One of the 180 woredas in the Oromia Region of Ethiopia. Part of the Arsi Zone, Robe is bordered on the south by the Shebelle River which separates it from the Bale Zone, on the southwest by Sherka, on the west by Tena, on the north by Sude, on the northeast by Amigna, and on the east by Seru. The woreda capital is Robe; other towns include Habe and Sedika.</obo:IAO_0000115>
        <oboInOwl:hasOBONamespace>GAZ</oboInOwl:hasOBONamespace>
        <oboInOwl:id>GAZ:00123753</oboInOwl:id>
        <rdfs:label>Robe Woreda</rdfs:label>
    </owl:NamedIndividual>
    


    <!-- http://purl.obolibrary.org/obo/GAZ_00123754 -->

    <owl:NamedIndividual rdf:about="http://purl.obolibrary.org/obo/GAZ_00123754">
        <obo:RO_0001025 rdf:resource="http://purl.obolibrary.org/obo/GAZ_00031114"/>
        <obo:IAO_0000115>One of the 180 woredas in the Oromia Region of Ethiopia; it is named after the woreda capital, Adaba. Part of the Bale Zone.</obo:IAO_0000115>
        <oboInOwl:hasOBONamespace>GAZ</oboInOwl:hasOBONamespace>
        <oboInOwl:id>GAZ:00123754</oboInOwl:id>
        <rdfs:label>Gasera Gololcha Woreda</rdfs:label>
    </owl:NamedIndividual>
    


    <!-- http://purl.obolibrary.org/obo/GAZ_00123755 -->

    <owl:NamedIndividual rdf:about="http://purl.obolibrary.org/obo/GAZ_00123755">
        <obo:RO_0001025 rdf:resource="http://purl.obolibrary.org/obo/GAZ_00031114"/>
        <obo:IAO_0000115>One of the 180 woredas in the Oromia Region of Ethiopia, named for the woreda capital, Agarfa. Located in the northwestern corner of the Bale Zone, Agarfa is bordered on the south by Sinanana Dinsho, on the west by Adaba, on the north by the Shabelle River which separates it from the Arsi Zone, and on the east by Gaserana Gololcha. Other towns in Agarfa include Ali.</obo:IAO_0000115>
        <oboInOwl:hasOBONamespace>GAZ</oboInOwl:hasOBONamespace>
        <oboInOwl:id>GAZ:00123755</oboInOwl:id>
        <rdfs:label>Agarfa Woreda</rdfs:label>
    </owl:NamedIndividual>
    


    <!-- http://purl.obolibrary.org/obo/GAZ_00123756 -->

    <owl:NamedIndividual rdf:about="http://purl.obolibrary.org/obo/GAZ_00123756">
        <obo:RO_0001025 rdf:resource="http://purl.obolibrary.org/obo/GAZ_00031114"/>
        <obo:IAO_0000115>One of the 180 woredas in the Oromia Region of Ethiopia. Part of the Bale Zone, Goro is bordered on the southwest by Guradamole, on the west by Berbere, on the northwest by Sinanana Dinsho, on the northeast by Ginir, and on the southeast by the Somali Region; it is separated from Guradamole and Berbere by the Gestro River.</obo:IAO_0000115>
        <oboInOwl:hasOBONamespace>GAZ</oboInOwl:hasOBONamespace>
        <oboInOwl:id>GAZ:00123756</oboInOwl:id>
        <rdfs:label>Goro Woreda</rdfs:label>
    </owl:NamedIndividual>
    


    <!-- http://purl.obolibrary.org/obo/GAZ_00123757 -->

    <owl:NamedIndividual rdf:about="http://purl.obolibrary.org/obo/GAZ_00123757">
        <obo:RO_0001025 rdf:resource="http://purl.obolibrary.org/obo/GAZ_00031114"/>
        <obo:IAO_0000115>One of the 180 woredas in the Oromia Region of Ethiopia. Part of the Bale Zone, Berbere is bordered on the south by Mennana Harena Buluk, on the northwest by Goba, on the north by Sinanana Dinsho, on the northeast by Goro, and on the east by Guradamole; the Mena River separates it from Shinanana Dinsho and Goro. The woreda capital is Haro Dumal.</obo:IAO_0000115>
        <oboInOwl:hasOBONamespace>GAZ</oboInOwl:hasOBONamespace>
        <oboInOwl:id>GAZ:00123757</oboInOwl:id>
        <rdfs:label>Berbere Woreda</rdfs:label>
    </owl:NamedIndividual>
    


    <!-- http://purl.obolibrary.org/obo/GAZ_00123758 -->

    <owl:NamedIndividual rdf:about="http://purl.obolibrary.org/obo/GAZ_00123758">
        <obo:RO_0001025 rdf:resource="http://purl.obolibrary.org/obo/GAZ_00031114"/>
        <obo:IAO_0000115>One of the 180 woredas in the Oromia Region of Ethiopia. Part of the Bale Zone, Ginir is bordered on the south by the Gestro River which separates it from Goro, on the west by Sinanana Dinsho, on the northwest by Gaserana Gololcha, on the northeast by Seweyna, and on the east by Raytu. Towns include Delo Serbo.</obo:IAO_0000115>
        <oboInOwl:hasOBONamespace>GAZ</oboInOwl:hasOBONamespace>
        <oboInOwl:id>GAZ:00123758</oboInOwl:id>
        <rdfs:label>Ginir Woreda</rdfs:label>
    </owl:NamedIndividual>
    


    <!-- http://purl.obolibrary.org/obo/GAZ_00123759 -->

    <owl:NamedIndividual rdf:about="http://purl.obolibrary.org/obo/GAZ_00123759">
        <obo:RO_0001025 rdf:resource="http://purl.obolibrary.org/obo/GAZ_00031114"/>
        <obo:IAO_0000115>One of the 180 woredas in the Oromia Region of Ethiopia; it is named after the woreda capital, Dodola. Part of the Bale Zone, Dodola is bordered on the south by Nensebo, on the west by Kokosa, on the north by the Shebelle River which separates it from the Arsi Zone, and on the east by Adaba. Other towns include Herero.</obo:IAO_0000115>
        <oboInOwl:hasOBONamespace>GAZ</oboInOwl:hasOBONamespace>
        <oboInOwl:id>GAZ:00123759</oboInOwl:id>
        <rdfs:label>Dodola Woreda</rdfs:label>
    </owl:NamedIndividual>
    


    <!-- http://purl.obolibrary.org/obo/GAZ_00123760 -->

    <owl:NamedIndividual rdf:about="http://purl.obolibrary.org/obo/GAZ_00123760">
        <obo:RO_0001025 rdf:resource="http://purl.obolibrary.org/obo/GAZ_00031114"/>
        <obo:IAO_0000115>One of the 180 woredas in the Oromia Region of Ethiopia. Part of the Bale Zone, Nensebo is bordered on the south by the Borena Zone, on the west by the Southern Nations, Nationalities and Peoples Region, on the northwest by Kokosa, on the north by Dodola, on the northeast by Adaba, on the east by Mennana Harena Buluk, and on the southeast by Meda Welabu. Towns in Nensebo include Werka.</obo:IAO_0000115>
        <oboInOwl:hasOBONamespace>GAZ</oboInOwl:hasOBONamespace>
        <oboInOwl:id>GAZ:00123760</oboInOwl:id>
        <rdfs:label>Nensebo Woreda</rdfs:label>
    </owl:NamedIndividual>
    


    <!-- http://purl.obolibrary.org/obo/GAZ_00123761 -->

    <owl:NamedIndividual rdf:about="http://purl.obolibrary.org/obo/GAZ_00123761">
        <obo:RO_0001025 rdf:resource="http://purl.obolibrary.org/obo/GAZ_00031114"/>
        <obo:IAO_0000115>One of the 180 woredas in the Oromia Region of Ethiopia. Located in the eastern part of the Bale Zone, Seweyna is bordered on the south by Raytu, on the southwest by Ginir, on the northwest by Gaserana Gololcha, on the north by Legehida, and on the east by the Somali Region. Towns in Seweyna include Hada.</obo:IAO_0000115>
        <oboInOwl:hasOBONamespace>GAZ</oboInOwl:hasOBONamespace>
        <oboInOwl:id>GAZ:00123761</oboInOwl:id>
        <rdfs:label>Seweyna Woreda</rdfs:label>
    </owl:NamedIndividual>
    


    <!-- http://purl.obolibrary.org/obo/GAZ_00123762 -->

    <owl:NamedIndividual rdf:about="http://purl.obolibrary.org/obo/GAZ_00123762">
        <obo:RO_0001025 rdf:resource="http://purl.obolibrary.org/obo/GAZ_00031114"/>
        <obo:IAO_0000115>One of the 180 woredas in the Oromia Region of Ethiopia. Located at the westernmost point of the Bale Zone, Kokosa is bordered on the south and west by the Southern Nations, Nationalities and Peoples Region, on the north by the Arsi Zone, on the northeast by Dodola, and on the southeast by Nensebo. The woreda capital is Nensebo; other towns include Kokosa.</obo:IAO_0000115>
        <oboInOwl:hasOBONamespace>GAZ</oboInOwl:hasOBONamespace>
        <oboInOwl:id>GAZ:00123762</oboInOwl:id>
        <rdfs:label>Kokosa Woreda</rdfs:label>
    </owl:NamedIndividual>
    


    <!-- http://purl.obolibrary.org/obo/GAZ_00123763 -->

    <owl:NamedIndividual rdf:about="http://purl.obolibrary.org/obo/GAZ_00123763">
        <obo:RO_0001025 rdf:resource="http://purl.obolibrary.org/obo/GAZ_00031114"/>
        <obo:IAO_0000115>One of the 180 woredas in the Oromia Region of Ethiopia. Part of the Bale Zone, Meda Welabu is bordered on the south by the Ganale Dorya River which separates it from the Borena Zone, on the northwest by Nensebo, on the north by Mennana Harena Buluk, and on the northeast by Guradamole. The woreda capital is Bidire.</obo:IAO_0000115>
        <oboInOwl:hasOBONamespace>GAZ</oboInOwl:hasOBONamespace>
        <oboInOwl:id>GAZ:00123763</oboInOwl:id>
        <rdfs:label>Meda Welabu Woreda</rdfs:label>
    </owl:NamedIndividual>
    


    <!-- http://purl.obolibrary.org/obo/GAZ_00123764 -->

    <owl:NamedIndividual rdf:about="http://purl.obolibrary.org/obo/GAZ_00123764">
        <obo:RO_0001025 rdf:resource="http://purl.obolibrary.org/obo/GAZ_00031114"/>
        <obo:IAO_0000115>One of the 180 woredas in the Oromia Region of Ethiopia. Part of the Bale Zone, Legehida is bordered on the south by Seweyna, on the southwest by Gaserana Gololcha, and all other sides by the Shebelle River which separates this woreda from the Mirab Hararghe Zone on the northwest, the Misraq Hararghe Zone on the northeast and from the Somali Region on the east. The woreda capital is Beltu; other towns include Sheikh Hussein.</obo:IAO_0000115>
        <oboInOwl:hasOBONamespace>GAZ</oboInOwl:hasOBONamespace>
        <oboInOwl:id>GAZ:00123764</oboInOwl:id>
        <rdfs:label>Legehida Woreda</rdfs:label>
    </owl:NamedIndividual>
    


    <!-- http://purl.obolibrary.org/obo/GAZ_00123765 -->

    <owl:NamedIndividual rdf:about="http://purl.obolibrary.org/obo/GAZ_00123765">
        <obo:RO_0001025 rdf:resource="http://purl.obolibrary.org/obo/GAZ_00031114"/>
        <obo:IAO_0000115>One of the 180 woredas in the Oromia Region of Ethiopia; it is named after the woreda capital, Adaba. Part of the Bale Zone, Adaba is bordered on the south by Mennana Harena Buluk, on the southwest by Nensebo, on the west by Dodola, on the northwest by the Shabelle River which separates it from the Arsi Zone, on the northeast by Agarfa, on the east by Sinanana Dinsho, and on the southeast by Goba.</obo:IAO_0000115>
        <oboInOwl:hasOBONamespace>GAZ</oboInOwl:hasOBONamespace>
        <oboInOwl:id>GAZ:00123765</oboInOwl:id>
        <rdfs:label>Adaba Woreda</rdfs:label>
    </owl:NamedIndividual>
    


    <!-- http://purl.obolibrary.org/obo/GAZ_00123766 -->

    <owl:NamedIndividual rdf:about="http://purl.obolibrary.org/obo/GAZ_00123766">
        <obo:RO_0001025 rdf:resource="http://purl.obolibrary.org/obo/GAZ_00031114"/>
        <obo:IAO_0000115>One of the 180 woredas in the Oromia Region of Ethiopia; it is named after the woreda capital, Adaba. Part of the Bale Zone.</obo:IAO_0000115>
        <oboInOwl:hasOBONamespace>GAZ</oboInOwl:hasOBONamespace>
        <oboInOwl:id>GAZ:00123766</oboInOwl:id>
        <rdfs:label>Guradamole Woreda</rdfs:label>
    </owl:NamedIndividual>
    


    <!-- http://purl.obolibrary.org/obo/GAZ_00123767 -->

    <owl:NamedIndividual rdf:about="http://purl.obolibrary.org/obo/GAZ_00123767">
        <obo:RO_0001025 rdf:resource="http://purl.obolibrary.org/obo/GAZ_00031114"/>
        <obo:IAO_0000115>One of the 180 woredas in the Oromia Region of Ethiopia. Located in the eastern part of the Bale Zone, Raytu is bordered on the south by the Somali Region, on the west by Ginir, and on the north and east by Seweyna; the Gestro River defines the southwest boundary. Towns in Raytu include Tedecha Bela&apos;a.</obo:IAO_0000115>
        <oboInOwl:hasOBONamespace>GAZ</oboInOwl:hasOBONamespace>
        <oboInOwl:id>GAZ:00123767</oboInOwl:id>
        <rdfs:label>Raytu Woreda</rdfs:label>
    </owl:NamedIndividual>
    


    <!-- http://purl.obolibrary.org/obo/GAZ_00123768 -->

    <owl:NamedIndividual rdf:about="http://purl.obolibrary.org/obo/GAZ_00123768">
        <obo:RO_0001025 rdf:resource="http://purl.obolibrary.org/obo/GAZ_00031114"/>
        <obo:IAO_0000115>One of the 180 woredas in the Oromia Region of Ethiopia. Part of the Bale Zone, Goba is bordered on the south by Mennana Harena Buluk, on the west by Adaba, on the north by the Mena River which separates it from Sinanana Dinsho, and on the southeast by Berbere.</obo:IAO_0000115>
        <oboInOwl:hasOBONamespace>GAZ</oboInOwl:hasOBONamespace>
        <oboInOwl:id>GAZ:00123768</oboInOwl:id>
        <rdfs:label>Goba Woreda</rdfs:label>
    </owl:NamedIndividual>
    


    <!-- http://purl.obolibrary.org/obo/GAZ_00123769 -->

    <owl:NamedIndividual rdf:about="http://purl.obolibrary.org/obo/GAZ_00123769">
        <obo:RO_0001025 rdf:resource="http://purl.obolibrary.org/obo/GAZ_00031114"/>
        <obo:IAO_0000115>One of the 180 woredas in the Oromia Region of Ethiopia; it is named after the woreda capital, Adaba. Part of the Bale Zone.</obo:IAO_0000115>
        <oboInOwl:hasOBONamespace>GAZ</oboInOwl:hasOBONamespace>
        <oboInOwl:id>GAZ:00123769</oboInOwl:id>
        <rdfs:label>Menna Harena Buluk Woreda</rdfs:label>
    </owl:NamedIndividual>
    


    <!-- http://purl.obolibrary.org/obo/GAZ_00123770 -->

    <owl:NamedIndividual rdf:about="http://purl.obolibrary.org/obo/GAZ_00123770">
        <obo:RO_0001025 rdf:resource="http://purl.obolibrary.org/obo/GAZ_00031113"/>
        <obo:IAO_0000115>One of the 180 woredas in the Oromia Region of Ethiopia. Located in the southern part of the Borena Zone, Dire is bordered on the south by Kenya, on the west by Teltele, on the north by Yabelo, on the northeast by Arero, and on the east by Moyale. Towns in Dire include Mega and Hidi Lola.</obo:IAO_0000115>
        <oboInOwl:hasOBONamespace>GAZ</oboInOwl:hasOBONamespace>
        <oboInOwl:id>GAZ:00123770</oboInOwl:id>
        <rdfs:label>Dire Woreda</rdfs:label>
    </owl:NamedIndividual>
    


    <!-- http://purl.obolibrary.org/obo/GAZ_00123771 -->

    <owl:NamedIndividual rdf:about="http://purl.obolibrary.org/obo/GAZ_00123771">
        <obo:RO_0001025 rdf:resource="http://purl.obolibrary.org/obo/GAZ_00031113"/>
        <obo:IAO_0000115>One of the 180 woredas in the Oromia Region of Ethiopia. Part of the Borena Zone, Arero is bordered on the southwest by Dire, on the west by Yabelo, on the north by Hagere Mariam, on the northeast by Odo Shakiso, on the east by Liben, and on the southeast by Moyale; the Dawa River, the only river in this woreda, separate Arero from Odo Shakiso and Liben. Towns in Arero include Meta Gefersa.</obo:IAO_0000115>
        <oboInOwl:hasOBONamespace>GAZ</oboInOwl:hasOBONamespace>
        <oboInOwl:id>GAZ:00123771</oboInOwl:id>
        <rdfs:label>Arero Woreda</rdfs:label>
    </owl:NamedIndividual>
    


    <!-- http://purl.obolibrary.org/obo/GAZ_00123772 -->

    <owl:NamedIndividual rdf:about="http://purl.obolibrary.org/obo/GAZ_00123772">
        <obo:RO_0001025 rdf:resource="http://purl.obolibrary.org/obo/GAZ_00031113"/>
        <obo:IAO_0000115>One of the 180 woredas in the Oromia Region of Ethiopia. Part of the Borena Zone, Hagere Mariam is bordered on the south by the Dawa River which separates it from Arero, on the southwest by Yabelo, on the west by the Southern Nations, Nationalities, and Peoples Region and Gelana Abaya, on the northeast by Uraga, and on the east by Odo Shakiso. Towns in Hagere Mariam include Hagere Mariam.</obo:IAO_0000115>
        <oboInOwl:hasOBONamespace>GAZ</oboInOwl:hasOBONamespace>
        <oboInOwl:id>GAZ:00123772</oboInOwl:id>
        <rdfs:label>Hagere Mariam Woreda</rdfs:label>
    </owl:NamedIndividual>
    


    <!-- http://purl.obolibrary.org/obo/GAZ_00123773 -->

    <owl:NamedIndividual rdf:about="http://purl.obolibrary.org/obo/GAZ_00123773">
        <obo:RO_0001025 rdf:resource="http://purl.obolibrary.org/obo/GAZ_00031113"/>
        <obo:IAO_0000115>One of the 180 woredas in the Oromia Region of Ethiopia. Part of the Borena Zone, Liben is bordered on the south by the Dawa River which separates it from Moyale and Arero, on the west by Odo Shakiso, on the northwest by Adolana Wadera, on the north by the Ganale Dorya River which separates it from the Bale Zone, and on the east by the Somali Region. The administrative center is Negele Boran; other towns in Liben include Hare Kalo.</obo:IAO_0000115>
        <oboInOwl:hasOBONamespace>GAZ</oboInOwl:hasOBONamespace>
        <oboInOwl:id>GAZ:00123773</oboInOwl:id>
        <rdfs:label>Liben Woreda</rdfs:label>
    </owl:NamedIndividual>
    


    <!-- http://purl.obolibrary.org/obo/GAZ_00123774 -->

    <owl:NamedIndividual rdf:about="http://purl.obolibrary.org/obo/GAZ_00123774">
        <obo:RO_0001025 rdf:resource="http://purl.obolibrary.org/obo/GAZ_00031113"/>
        <obo:IAO_0000115>One of the 180 woredas in the Oromia Region of Ethiopia. Part of the Borena Zone, Adolana Wadera is bordered on the south by Liben, on the southwest by Odo Shakiso, on the west by Bore, on the north by the Southern Nations, Nationalities, and Peoples Region, and on the east by the Bale Zone. Towns in Adolana Wadera include Kebri Mangest and Wadera.</obo:IAO_0000115>
        <oboInOwl:hasOBONamespace>GAZ</oboInOwl:hasOBONamespace>
        <oboInOwl:id>GAZ:00123774</oboInOwl:id>
        <rdfs:label>Adolana Wadera Woreda</rdfs:label>
    </owl:NamedIndividual>
    


    <!-- http://purl.obolibrary.org/obo/GAZ_00123775 -->

    <owl:NamedIndividual rdf:about="http://purl.obolibrary.org/obo/GAZ_00123775">
        <obo:RO_0001025 rdf:resource="http://purl.obolibrary.org/obo/GAZ_00031113"/>
        <obo:IAO_0000115>One of the 180 woredas in the Oromia Region of Ethiopia. Part of the Borena Zone, Uraga is bordered on the south by Odo Shakiso, on the west by Hagere Mariam, on the north by the Southern Nations, Nationalities, and Peoples Region, and on the east by Bore. Towns in Uraga include Solomo.</obo:IAO_0000115>
        <oboInOwl:hasOBONamespace>GAZ</oboInOwl:hasOBONamespace>
        <oboInOwl:id>GAZ:00123775</oboInOwl:id>
        <rdfs:label>Uraga Woreda</rdfs:label>
    </owl:NamedIndividual>
    


    <!-- http://purl.obolibrary.org/obo/GAZ_00123776 -->

    <owl:NamedIndividual rdf:about="http://purl.obolibrary.org/obo/GAZ_00123776">
        <obo:RO_0001025 rdf:resource="http://purl.obolibrary.org/obo/GAZ_00031113"/>
        <obo:IAO_0000115>One of the 180 woredas in the Oromia Region of Ethiopia. Located in the southeast corner of the Borena Zone, Moyale is bordered on the south by Kenya, on the west by Dire, on the northwest by Arero, on the north by the Dawa River which separates it from Liben, and on the east by the Somali Region.</obo:IAO_0000115>
        <oboInOwl:hasOBONamespace>GAZ</oboInOwl:hasOBONamespace>
        <oboInOwl:id>GAZ:00123776</oboInOwl:id>
        <rdfs:label>Moyale Woreda</rdfs:label>
    </owl:NamedIndividual>
    


    <!-- http://purl.obolibrary.org/obo/GAZ_00123777 -->

    <owl:NamedIndividual rdf:about="http://purl.obolibrary.org/obo/GAZ_00123777">
        <obo:RO_0001025 rdf:resource="http://purl.obolibrary.org/obo/GAZ_00031113"/>
        <obo:IAO_0000115>One of the 180 woredas in the Oromia Region of Ethiopia. Part of the Borena Zone, Odo Shakiso is bordered on the south by the Dawa River which separates it from Arero, on the west by Hagere Mariam, on the northeast by Uraga, on the north by Bore, on the northeast by Adolana Wadera, and on the east by Liben. Towns in Odo Shakiso include Shakiso and Megado.</obo:IAO_0000115>
        <oboInOwl:hasOBONamespace>GAZ</oboInOwl:hasOBONamespace>
        <oboInOwl:id>GAZ:00123777</oboInOwl:id>
        <rdfs:label>Odo Shakiso Woreda</rdfs:label>
    </owl:NamedIndividual>
    


    <!-- http://purl.obolibrary.org/obo/GAZ_00123778 -->

    <owl:NamedIndividual rdf:about="http://purl.obolibrary.org/obo/GAZ_00123778">
        <obo:RO_0001025 rdf:resource="http://purl.obolibrary.org/obo/GAZ_00031113"/>
        <obo:IAO_0000115>One of the 180 woredas in the Oromia Region of Ethiopia. Located in the northern part of the Borena Zone, Bore is bordered on the south by Odo Shakiso, on the west by Uraga, on the north by the Southern Nations, Nationalities, and Peoples Region, and on the east by Adolana Wadera. Towns in Bore include Bore and Yirba Muda.</obo:IAO_0000115>
        <oboInOwl:hasOBONamespace>GAZ</oboInOwl:hasOBONamespace>
        <oboInOwl:id>GAZ:00123778</oboInOwl:id>
        <rdfs:label>Bore Woreda</rdfs:label>
    </owl:NamedIndividual>
    


    <!-- http://purl.obolibrary.org/obo/GAZ_00123779 -->

    <owl:NamedIndividual rdf:about="http://purl.obolibrary.org/obo/GAZ_00123779">
        <obo:RO_0001025 rdf:resource="http://purl.obolibrary.org/obo/GAZ_00031113"/>
        <obo:IAO_0000115>One of the 180 woredas in the Oromia Region of Ethiopia. Part of the Borena Zone, Gelana Abaya is bordered on the south by Hagere Mariam, and on the west, north and east by the Southern Nations, Nationalities, and Peoples Region (SNNPR). Lake Abaya, on the western border, is divided between this woreda and the SNNPR.</obo:IAO_0000115>
        <oboInOwl:hasOBONamespace>GAZ</oboInOwl:hasOBONamespace>
        <oboInOwl:id>GAZ:00123779</oboInOwl:id>
        <rdfs:label>Gelana Abaya Woreda</rdfs:label>
    </owl:NamedIndividual>
    


    <!-- http://purl.obolibrary.org/obo/GAZ_00123780 -->

    <owl:NamedIndividual rdf:about="http://purl.obolibrary.org/obo/GAZ_00123780">
        <obo:RO_0001025 rdf:resource="http://purl.obolibrary.org/obo/GAZ_00031113"/>
        <obo:IAO_0000115>One of the 180 woredas in the Oromia Region of Ethiopia. It is named after the administrative center, Teltele. Located in the southwest corner of the Borena Zone, Teltele is bordered on the southwest by Kenya, on the west and north by the Sagan River, the only river in this woreda, which separates it from the Southern Nations, Nationalities, and Peoples Region, on the northeast by Yabelo, and on the southeast by Dire.</obo:IAO_0000115>
        <oboInOwl:hasOBONamespace>GAZ</oboInOwl:hasOBONamespace>
        <oboInOwl:id>GAZ:00123780</oboInOwl:id>
        <rdfs:label>Teltele Woreda</rdfs:label>
    </owl:NamedIndividual>
    


    <!-- http://purl.obolibrary.org/obo/GAZ_00123781 -->

    <owl:NamedIndividual rdf:about="http://purl.obolibrary.org/obo/GAZ_00123781">
        <obo:RO_0001025 rdf:resource="http://purl.obolibrary.org/obo/GAZ_00031120"/>
        <obo:IAO_0000115>One of the 180 woredas in the Oromia Region of Ethiopia. Part of the Illubabor Zone, Ale is bordered on the south by the Southern Nations, Nationalities and Peoples Region, on the west by Nono, on the northwest by Bure, and on the northeast by Metu. Towns in Ale include Ale, Gore and Leka.</obo:IAO_0000115>
        <oboInOwl:hasOBONamespace>GAZ</oboInOwl:hasOBONamespace>
        <oboInOwl:id>GAZ:00123781</oboInOwl:id>
        <rdfs:label>Ale Woreda</rdfs:label>
    </owl:NamedIndividual>
    


    <!-- http://purl.obolibrary.org/obo/GAZ_00123782 -->

    <owl:NamedIndividual rdf:about="http://purl.obolibrary.org/obo/GAZ_00123782">
        <obo:RO_0001025 rdf:resource="http://purl.obolibrary.org/obo/GAZ_00031120"/>
        <obo:IAO_0000115>One of the 180 woredas in the Oromia Region of Ethiopia. Part of the Illubabor Zone, Gechi is bordered on the south by Didessa, on the west by the Jimma Zone, on the north by Bedele, and on the east by the Didessa River which separates it from the Jimma Zone. Towns in Gechi include Gechi and Yanfu.</obo:IAO_0000115>
        <oboInOwl:hasOBONamespace>GAZ</oboInOwl:hasOBONamespace>
        <oboInOwl:id>GAZ:00123782</oboInOwl:id>
        <rdfs:label>Gechi Woreda</rdfs:label>
    </owl:NamedIndividual>
    


    <!-- http://purl.obolibrary.org/obo/GAZ_00123783 -->

    <owl:NamedIndividual rdf:about="http://purl.obolibrary.org/obo/GAZ_00123783">
        <obo:RO_0001025 rdf:resource="http://purl.obolibrary.org/obo/GAZ_00031120"/>
        <obo:IAO_0000115>One of the 180 woredas in the Oromia Region of Ethiopia. Part of the Illubabor Zone, Nono is bordered on the on the southwest by the Gambela Region, on the north by Bure, on the northeast by Ale, and on the southeast by the Southern Nations, Nationalities and Peoples Region. Towns in Nono include Birbirsa and Nono.</obo:IAO_0000115>
        <oboInOwl:hasOBONamespace>GAZ</oboInOwl:hasOBONamespace>
        <oboInOwl:id>GAZ:00123783</oboInOwl:id>
        <rdfs:label>Nono Woreda</rdfs:label>
    </owl:NamedIndividual>
    


    <!-- http://purl.obolibrary.org/obo/GAZ_00123784 -->

    <owl:NamedIndividual rdf:about="http://purl.obolibrary.org/obo/GAZ_00123784">
        <obo:RO_0001025 rdf:resource="http://purl.obolibrary.org/obo/GAZ_00031120"/>
        <obo:IAO_0000115>One of the 180 woredas in the Oromia Region of Ethiopia. Part of the Illubabor Zone, Darimu is bordered on the south by Metu, on the west and north by the Mirab Welega Zone, and on the east by Supena Sodo. The major town in Darimu is Dipa.</obo:IAO_0000115>
        <oboInOwl:hasOBONamespace>GAZ</oboInOwl:hasOBONamespace>
        <oboInOwl:id>GAZ:00123784</oboInOwl:id>
        <rdfs:label>Darimu Woreda</rdfs:label>
    </owl:NamedIndividual>
    


    <!-- http://purl.obolibrary.org/obo/GAZ_00123785 -->

    <owl:NamedIndividual rdf:about="http://purl.obolibrary.org/obo/GAZ_00123785">
        <obo:RO_0001025 rdf:resource="http://purl.obolibrary.org/obo/GAZ_00031120"/>
        <obo:IAO_0000115>One of the 180 woredas in the Oromia Region of Ethiopia. Part of the Illubabor Zone, Bure is bordered on the south by Nono, on the southwest by the Gambela Region, on the west by the Mirab Welega Zone, on the northeast by Metu, and on the southeast by Ale; the Birbir River defines the west and north boundaries. Towns in Bure include Bure and Sibo.</obo:IAO_0000115>
        <oboInOwl:hasOBONamespace>GAZ</oboInOwl:hasOBONamespace>
        <oboInOwl:id>GAZ:00123785</oboInOwl:id>
        <rdfs:label>Bure Woreda</rdfs:label>
    </owl:NamedIndividual>
    


    <!-- http://purl.obolibrary.org/obo/GAZ_00123786 -->

    <owl:NamedIndividual rdf:about="http://purl.obolibrary.org/obo/GAZ_00123786">
        <obo:RO_0001025 rdf:resource="http://purl.obolibrary.org/obo/GAZ_00031120"/>
        <obo:IAO_0000115>One of the 180 woredas in the Oromia Region of Ethiopia. It is named after the Didessa River, a tributary of the Abay River. Part of the Illubabor Zone, Didessa is bordered on the south by the Didessa River which separates it from the Jimma Zone, and on the north by Gechi. The major town in Dedesa is Denbi.</obo:IAO_0000115>
        <oboInOwl:hasOBONamespace>GAZ</oboInOwl:hasOBONamespace>
        <oboInOwl:id>GAZ:00123786</oboInOwl:id>
        <rdfs:label>Didessa Woreda</rdfs:label>
    </owl:NamedIndividual>
    


    <!-- http://purl.obolibrary.org/obo/GAZ_00123787 -->

    <owl:NamedIndividual rdf:about="http://purl.obolibrary.org/obo/GAZ_00123787">
        <obo:RO_0001025 rdf:resource="http://purl.obolibrary.org/obo/GAZ_00031120"/>
        <obo:IAO_0000115>One of the 180 woredas in the Oromia Region of Ethiopia. Part of the Illubabor Zone, Metu is bordered on the south by Ale, on the southwest by Bure, on the west by the Mirab Welega Zone, on the north by Darimu, on the northeast by Supena Sodo, on the east by Yayu and on the southeast by Southern Nations, Nationalities and Peoples Region. Towns in Metu include Metu and Nopa.</obo:IAO_0000115>
        <oboInOwl:hasOBONamespace>GAZ</oboInOwl:hasOBONamespace>
        <oboInOwl:id>GAZ:00123787</oboInOwl:id>
        <rdfs:label>Metu Woreda</rdfs:label>
    </owl:NamedIndividual>
    


    <!-- http://purl.obolibrary.org/obo/GAZ_00123788 -->

    <owl:NamedIndividual rdf:about="http://purl.obolibrary.org/obo/GAZ_00123788">
        <obo:RO_0001025 rdf:resource="http://purl.obolibrary.org/obo/GAZ_00031120"/>
        <obo:IAO_0000115>One of the 180 woredas in the Oromia Region of Ethiopia. Part of the Illubabor Zone, Dega is bordered on the south by Chora, on the west by Supena Sodo, on the north by the Mirab Welega Zone, on the northeast by the southern exclave of the Benishangul-Gumuz Region, and on the east by Bedele. Towns in Dega include Dega and Mako.</obo:IAO_0000115>
        <oboInOwl:hasOBONamespace>GAZ</oboInOwl:hasOBONamespace>
        <oboInOwl:id>GAZ:00123788</oboInOwl:id>
        <rdfs:label>Dega Woreda</rdfs:label>
    </owl:NamedIndividual>
    


    <!-- http://purl.obolibrary.org/obo/GAZ_00123789 -->

    <owl:NamedIndividual rdf:about="http://purl.obolibrary.org/obo/GAZ_00123789">
        <obo:RO_0001025 rdf:resource="http://purl.obolibrary.org/obo/GAZ_00031120"/>
        <obo:IAO_0000115>One of the 180 woredas in the Oromia Region of Ethiopia. Part of the Illubabor Zone, Supena Sodo is bordered on the south by Yayu, on the southwest by Metu, on the west by Darimu, on the north by the Mirab Welega Zone, on the northeast by Dega, and on the southeast by Chora. Towns in Supena Sodo include Alge, Sache and Supe.</obo:IAO_0000115>
        <oboInOwl:hasOBONamespace>GAZ</oboInOwl:hasOBONamespace>
        <oboInOwl:id>GAZ:00123789</oboInOwl:id>
        <rdfs:label>Supena Sodo Woreda</rdfs:label>
    </owl:NamedIndividual>
    


    <!-- http://purl.obolibrary.org/obo/GAZ_00123790 -->

    <owl:NamedIndividual rdf:about="http://purl.obolibrary.org/obo/GAZ_00123790">
        <obo:RO_0001025 rdf:resource="http://purl.obolibrary.org/obo/GAZ_00031120"/>
        <obo:IAO_0000115>One of the 180 woredas in the Oromia Region of Ethiopia. Part of the Illubabor Zone, Bedele is bordered on the south by Gechi, on the southwest by Chora, on the west by Dega, on the north by the southern exclave of the Benishangul-Gumuz Region, on the northeast by the Didessa River which separates it from the Misraq Welega Zone, and on the southeast by Gechi. Towns in Bedele include Bedele and Kone.</obo:IAO_0000115>
        <oboInOwl:hasOBONamespace>GAZ</oboInOwl:hasOBONamespace>
        <oboInOwl:id>GAZ:00123790</oboInOwl:id>
        <rdfs:label>Bedele Woreda</rdfs:label>
    </owl:NamedIndividual>
    


    <!-- http://purl.obolibrary.org/obo/GAZ_00123791 -->

    <owl:NamedIndividual rdf:about="http://purl.obolibrary.org/obo/GAZ_00123791">
        <obo:RO_0001025 rdf:resource="http://purl.obolibrary.org/obo/GAZ_00031120"/>
        <obo:IAO_0000115>One of the 180 woredas in the Oromia Region of Ethiopia. Part of the Illubabor Zone.</obo:IAO_0000115>
        <oboInOwl:hasOBONamespace>GAZ</oboInOwl:hasOBONamespace>
        <oboInOwl:id>GAZ:00123791</oboInOwl:id>
        <rdfs:label>Yayu Woreda</rdfs:label>
    </owl:NamedIndividual>
    


    <!-- http://purl.obolibrary.org/obo/GAZ_00123792 -->

    <owl:NamedIndividual rdf:about="http://purl.obolibrary.org/obo/GAZ_00123792">
        <obo:RO_0001025 rdf:resource="http://purl.obolibrary.org/obo/GAZ_00031120"/>
        <obo:IAO_0000115>One of the 180 woredas in the Oromia Region of Ethiopia. Part of the Illubabor Zone, Chora is bordered on the south by the Jimma Zone, on the west by Yayu, on the northwest by Supena Sodo, on the north by Dega, and on the east by Bedele. The major town in Chora is Kumbabe.</obo:IAO_0000115>
        <oboInOwl:hasOBONamespace>GAZ</oboInOwl:hasOBONamespace>
        <oboInOwl:id>GAZ:00123792</oboInOwl:id>
        <rdfs:label>Chora Woreda</rdfs:label>
    </owl:NamedIndividual>
    


    <!-- http://purl.obolibrary.org/obo/GAZ_00123793 -->

    <owl:NamedIndividual rdf:about="http://purl.obolibrary.org/obo/GAZ_00123793">
        <obo:RO_0001025 rdf:resource="http://purl.obolibrary.org/obo/GAZ_00031118"/>
        <obo:IAO_0000115>One of the 180 woredas in the Oromia Region of Ethiopia. Part of the Jimma Zone, Dedo is bordered on the south by the Gojeb River which separates it from the Southern Nations, Nationalities and Peoples Region, on the west by Gera, on the north by Kersa, and on the east by Omo Nada. The major town in Dedo is Sheki.</obo:IAO_0000115>
        <oboInOwl:hasOBONamespace>GAZ</oboInOwl:hasOBONamespace>
        <oboInOwl:id>GAZ:00123793</oboInOwl:id>
        <rdfs:label>Dedo Woreda</rdfs:label>
    </owl:NamedIndividual>
    


    <!-- http://purl.obolibrary.org/obo/GAZ_00123794 -->

    <owl:NamedIndividual rdf:about="http://purl.obolibrary.org/obo/GAZ_00123794">
        <obo:RO_0001025 rdf:resource="http://purl.obolibrary.org/obo/GAZ_00031118"/>
        <obo:IAO_0000115>One of the 180 woredas in the Oromia Region of Ethiopia. Located in the western part of the Jimma Zone, Setema is bordered on the south by Gera, on the west by Sigmo, on the north by the Illubabor Zone, and on the southeast by Gomma. The capital of the woreda is Gatira.</obo:IAO_0000115>
        <oboInOwl:hasOBONamespace>GAZ</oboInOwl:hasOBONamespace>
        <oboInOwl:id>GAZ:00123794</oboInOwl:id>
        <rdfs:label>Setema Woreda</rdfs:label>
    </owl:NamedIndividual>
    


    <!-- http://purl.obolibrary.org/obo/GAZ_00123795 -->

    <owl:NamedIndividual rdf:about="http://purl.obolibrary.org/obo/GAZ_00123795">
        <obo:RO_0001025 rdf:resource="http://purl.obolibrary.org/obo/GAZ_00031118"/>
        <obo:IAO_0000115>One of the 180 woredas in the Oromia Region of Ethiopia. Part of the Jimma Zone, Omo Nada is bordered on the south by the Gojeb River which separates it from the Southern Nations, Nationalities and Peoples Region (SNNPR), on the west by Dedo, on the northwest by Kersa, on the north by Tiro Afeta, on the northeast by Sokoru, and on the east by the Omo River which separates it from the SNNPR. Nada is the capital of the woreda; other towns in Omo Nada include Asendabo.</obo:IAO_0000115>
        <oboInOwl:hasOBONamespace>GAZ</oboInOwl:hasOBONamespace>
        <oboInOwl:id>GAZ:00123795</oboInOwl:id>
        <rdfs:label>Omo Nada Woreda</rdfs:label>
    </owl:NamedIndividual>
    


    <!-- http://purl.obolibrary.org/obo/GAZ_00123796 -->

    <owl:NamedIndividual rdf:about="http://purl.obolibrary.org/obo/GAZ_00123796">
        <obo:RO_0001025 rdf:resource="http://purl.obolibrary.org/obo/GAZ_00031118"/>
        <obo:IAO_0000115>One of the 180 woredas in the Oromia Region of Ethiopia. Part of the Jimma Zone, Limmu Kosa is bordered on the south by Kersa, on the southwest by Mana, on the west by Gomma, on the northwest by the Didessa River which separates it from the Illubabor Zone, on the north by Limmu Sakka, on the northeast by the Gibe River which separates it from the Mirab Shewa Zone and the Southern Nations, Nationalities and Peoples Region, on the east by Sokoru, and on the southeast by Tiro Afeta. The capital of this woreda is Genet; other towns include Ambuye and Babu.</obo:IAO_0000115>
        <oboInOwl:hasOBONamespace>GAZ</oboInOwl:hasOBONamespace>
        <oboInOwl:id>GAZ:00123796</oboInOwl:id>
        <rdfs:label>Limmu Kosa Woreda</rdfs:label>
    </owl:NamedIndividual>
    


    <!-- http://purl.obolibrary.org/obo/GAZ_00123797 -->

    <owl:NamedIndividual rdf:about="http://purl.obolibrary.org/obo/GAZ_00123797">
        <obo:RO_0001025 rdf:resource="http://purl.obolibrary.org/obo/GAZ_00031118"/>
        <obo:IAO_0000115>One of the 180 woredas in the Oromia Region of Ethiopia. Part of the Jimma Zone, Seka Chekorsa is bordered on the south by the Gojeb River which separates it from the Southern Nations, Nationalities and Peoples Region, on the west by Gera, on the northwest by Gomma, on the north by Mana, on the northeast by Kersa, and on the east by Dedo. Towns in this woreda include Shebe; villages include Bedadi.</obo:IAO_0000115>
        <oboInOwl:hasOBONamespace>GAZ</oboInOwl:hasOBONamespace>
        <oboInOwl:id>GAZ:00123797</oboInOwl:id>
        <rdfs:label>Seka Chekorsa Woreda</rdfs:label>
    </owl:NamedIndividual>
    


    <!-- http://purl.obolibrary.org/obo/GAZ_00123798 -->

    <owl:NamedIndividual rdf:about="http://purl.obolibrary.org/obo/GAZ_00123798">
        <obo:RO_0001025 rdf:resource="http://purl.obolibrary.org/obo/GAZ_00031118"/>
        <obo:IAO_0000115>One of the 180 woredas in the Oromia Region of Ethiopia. Part of the Jimma Zone, Sokoru is bordered on the south by Omo Nada, on the west by Tiro Afeta, and on the north and east by the Southern Nations, Nationalities and Peoples Region; the Gibe River defines the northern boundary. Besides the capital, other towns in this woreda include Deneba, Kumbi and Natri.</obo:IAO_0000115>
        <oboInOwl:hasOBONamespace>GAZ</oboInOwl:hasOBONamespace>
        <oboInOwl:id>GAZ:00123798</oboInOwl:id>
        <rdfs:label>Sokoru Woreda</rdfs:label>
    </owl:NamedIndividual>
    


    <!-- http://purl.obolibrary.org/obo/GAZ_00123799 -->

    <owl:NamedIndividual rdf:about="http://purl.obolibrary.org/obo/GAZ_00123799">
        <obo:RO_0001025 rdf:resource="http://purl.obolibrary.org/obo/GAZ_00031118"/>
        <obo:IAO_0000115>One of the 180 woredas in the Oromia Region of Ethiopia. Part of the Jimma Zone, Gomma is bordered on the south by Seka Chekorsa, on the southwest by Gera, on the northwest by Setema, on the north by the Didessa River which separates it from the Illubabor Zone, on the northeast by Limmu Kosa, and on the east by Mana. The administrative center of this woreda is Agaro; other towns include Beshasha, Choche, Ghembe, Limmu Shaye, and Toba.</obo:IAO_0000115>
        <oboInOwl:hasOBONamespace>GAZ</oboInOwl:hasOBONamespace>
        <oboInOwl:id>GAZ:00123799</oboInOwl:id>
        <rdfs:label>Gomma Woreda</rdfs:label>
    </owl:NamedIndividual>
    


    <!-- http://purl.obolibrary.org/obo/GAZ_00123800 -->

    <owl:NamedIndividual rdf:about="http://purl.obolibrary.org/obo/GAZ_00123800">
        <obo:RO_0001025 rdf:resource="http://purl.obolibrary.org/obo/GAZ_00031118"/>
        <oboInOwl:hasOBONamespace>GAZ</oboInOwl:hasOBONamespace>
        <oboInOwl:id>GAZ:00123800</oboInOwl:id>
        <rdfs:label>Tiro Afeta Woreda</rdfs:label>
    </owl:NamedIndividual>
    


    <!-- http://purl.obolibrary.org/obo/GAZ_00123801 -->

    <owl:NamedIndividual rdf:about="http://purl.obolibrary.org/obo/GAZ_00123801">
        <obo:RO_0001025 rdf:resource="http://purl.obolibrary.org/obo/GAZ_00031118"/>
        <obo:IAO_0000115>One of the 180 woredas in the Oromia Region of Ethiopia. Part of the Jimma Zone, Gera is bordered on the south by the Gojeb River which separates it from the Southern Nations, Nationalities and Peoples Region, on the northwest by Sigmo, on the north by Setema, on the northeast by Gomma, and on the east by Seka Chekorsa. The woreda capital is Chira; other towns include Cheriko and Dusta.</obo:IAO_0000115>
        <oboInOwl:hasOBONamespace>GAZ</oboInOwl:hasOBONamespace>
        <oboInOwl:id>GAZ:00123801</oboInOwl:id>
        <rdfs:label>Gera Woreda</rdfs:label>
    </owl:NamedIndividual>
    


    <!-- http://purl.obolibrary.org/obo/GAZ_00123802 -->

    <owl:NamedIndividual rdf:about="http://purl.obolibrary.org/obo/GAZ_00123802">
        <obo:RO_0001025 rdf:resource="http://purl.obolibrary.org/obo/GAZ_00031118"/>
        <obo:IAO_0000115>One of the 180 woredas in the Oromia Region of Ethiopia. This woreda is named after its capital, Sigmo. Located in the western part of the Jimma Zone, Sigmo is bordered on the south by Gera, on the west by the Southern Nations, Nationalities and Peoples Region, on the north by the Illubabor Zone, and on the east by Setema.</obo:IAO_0000115>
        <oboInOwl:hasOBONamespace>GAZ</oboInOwl:hasOBONamespace>
        <oboInOwl:id>GAZ:00123802</oboInOwl:id>
        <rdfs:label>Sigmo Woreda</rdfs:label>
    </owl:NamedIndividual>
    


    <!-- http://purl.obolibrary.org/obo/GAZ_00123803 -->

    <owl:NamedIndividual rdf:about="http://purl.obolibrary.org/obo/GAZ_00123803">
        <obo:RO_0001025 rdf:resource="http://purl.obolibrary.org/obo/GAZ_00031118"/>
        <obo:IAO_0000115>One of the 180 woredas in the Oromia Region of Ethiopia. Part of the Jimma Zone, Mana is bordered on the south by Seka Chekorsa, on the west by Gomma, on the north by Limmu Kosa, and on the east by Kersa. The administrative center of the woreda is Yebu.</obo:IAO_0000115>
        <oboInOwl:hasOBONamespace>GAZ</oboInOwl:hasOBONamespace>
        <oboInOwl:id>GAZ:00123803</oboInOwl:id>
        <rdfs:label>Mana Woreda</rdfs:label>
    </owl:NamedIndividual>
    


    <!-- http://purl.obolibrary.org/obo/GAZ_00123804 -->

    <owl:NamedIndividual rdf:about="http://purl.obolibrary.org/obo/GAZ_00123804">
        <obo:RO_0001025 rdf:resource="http://purl.obolibrary.org/obo/GAZ_00031118"/>
        <obo:IAO_0000115>One of the 180 woredas in the Oromia Region of Ethiopia. Part of the Jimma Zone, Limmu Sakka is bordered on the southwest by the Didessa River which separates it from the Illubabor Zone, on the northwest by the Misraq Welega Zone, on the northeast by the Mirab Shewa Zone, and on the southeast by Limmu Kosa. The administrative center of the woreda is Atnago; other towns include Saqqa, the capital of the former kingdom of Limmu-Ennarea.</obo:IAO_0000115>
        <oboInOwl:hasOBONamespace>GAZ</oboInOwl:hasOBONamespace>
        <oboInOwl:id>GAZ:00123804</oboInOwl:id>
        <rdfs:label>Limmu Sakka Woreda</rdfs:label>
    </owl:NamedIndividual>
    


    <!-- http://purl.obolibrary.org/obo/GAZ_00123805 -->

    <owl:NamedIndividual rdf:about="http://purl.obolibrary.org/obo/GAZ_00123805">
        <obo:RO_0001025 rdf:resource="http://purl.obolibrary.org/obo/GAZ_00031124"/>
        <obo:IAO_0000115>One of the 180 woredas in the Oromia Region of Ethiopia. Part of the Mirab Hararghe Zone, Boke is bordered on the south by the Shabelle River which separates it from the Bale Zone, on the southwest by Darolebu, on the northwest by Habro, on the northeast by Kuni, and on the east by the Galetti River which separates it from the Misraq Hararghe Zone. The major town in Boke is Boke Tiko.</obo:IAO_0000115>
        <oboInOwl:hasOBONamespace>GAZ</oboInOwl:hasOBONamespace>
        <oboInOwl:id>GAZ:00123805</oboInOwl:id>
        <rdfs:label>Boke Woreda</rdfs:label>
    </owl:NamedIndividual>
    


    <!-- http://purl.obolibrary.org/obo/GAZ_00123806 -->

    <owl:NamedIndividual rdf:about="http://purl.obolibrary.org/obo/GAZ_00123806">
        <obo:RO_0001025 rdf:resource="http://purl.obolibrary.org/obo/GAZ_00031124"/>
        <obo:IAO_0000115>One of the 180 woredas in the Oromia Region of Ethiopia. Part of the Mirab Hararghe Zone, Kuni is bordered on the south by Boke, on the west by Habro, on the northeast by Chiro, and on the east by the Galetti River which separates it from the Misraq Hararghe Zone. The major town in Kuni is Bedesa.</obo:IAO_0000115>
        <oboInOwl:hasOBONamespace>GAZ</oboInOwl:hasOBONamespace>
        <oboInOwl:id>GAZ:00123806</oboInOwl:id>
        <rdfs:label>Kuni Woreda</rdfs:label>
    </owl:NamedIndividual>
    


    <!-- http://purl.obolibrary.org/obo/GAZ_00123807 -->

    <owl:NamedIndividual rdf:about="http://purl.obolibrary.org/obo/GAZ_00123807">
        <obo:RO_0001025 rdf:resource="http://purl.obolibrary.org/obo/GAZ_00031124"/>
        <obo:IAO_0000115>One of the 180 woredas in the Oromia Region of Ethiopia. Part of the Mirab Hararghe Zone, Mesela is bordered on the southwest by the Galetti River which separates it from Chiro, on the northwest by Tulo, and on the east by the Misraq Hararghe Zone. Towns in Mesela include Goro Reye and Mesela.</obo:IAO_0000115>
        <oboInOwl:hasOBONamespace>GAZ</oboInOwl:hasOBONamespace>
        <oboInOwl:id>GAZ:00123807</oboInOwl:id>
        <rdfs:label>Mesela Woreda</rdfs:label>
    </owl:NamedIndividual>
    


    <!-- http://purl.obolibrary.org/obo/GAZ_00123808 -->

    <owl:NamedIndividual rdf:about="http://purl.obolibrary.org/obo/GAZ_00123808">
        <obo:RO_0001025 rdf:resource="http://purl.obolibrary.org/obo/GAZ_00031124"/>
        <obo:IAO_0000115>One of the 180 woredas in the Oromia Region of Ethiopia. Part of the Mirab Hararghe Zone, Mieso is bordered on the south by Guba Koricha, on the west by the Afar Region, on the north by the Somali Region, on the east by Doba and on the southeast by Chiro. Towns in Mieso include Arba Bordode, Asabot, Kora, Mieso and Mulu.</obo:IAO_0000115>
        <oboInOwl:hasOBONamespace>GAZ</oboInOwl:hasOBONamespace>
        <oboInOwl:id>GAZ:00123808</oboInOwl:id>
        <rdfs:label>Mieso Woreda</rdfs:label>
    </owl:NamedIndividual>
    


    <!-- http://purl.obolibrary.org/obo/GAZ_00123809 -->

    <owl:NamedIndividual rdf:about="http://purl.obolibrary.org/obo/GAZ_00123809">
        <obo:RO_0001025 rdf:resource="http://purl.obolibrary.org/obo/GAZ_00031124"/>
        <obo:IAO_0000115>One of the 180 woredas in the Oromia Region of Ethiopia. Part of the Mirab Hararghe Zone, Tulo is bordered on the south by Mesela, on the west by Chiro, on the north by Doba, and on the east by the Misraq Hararghe Zone. Towns in Tulo include Debeso and Hirna.</obo:IAO_0000115>
        <oboInOwl:hasOBONamespace>GAZ</oboInOwl:hasOBONamespace>
        <oboInOwl:id>GAZ:00123809</oboInOwl:id>
        <rdfs:label>Tulo Woreda</rdfs:label>
    </owl:NamedIndividual>
    


    <!-- http://purl.obolibrary.org/obo/GAZ_00123810 -->

    <owl:NamedIndividual rdf:about="http://purl.obolibrary.org/obo/GAZ_00123810">
        <obo:RO_0001025 rdf:resource="http://purl.obolibrary.org/obo/GAZ_00031124"/>
        <obo:IAO_0000115>One of the 180 woredas in the Oromia Region of Ethiopia. It is named after the former awraja of the same name. Part of the Mirab Hararghe Zone, Habro is bordered on the south by Darolebu, on the west and north by Guba Koricha, on the northeast by Kuni, and on the southeast by Boke. Towns in Habro include Belbelti, Gelemso and Wachu.</obo:IAO_0000115>
        <oboInOwl:hasOBONamespace>GAZ</oboInOwl:hasOBONamespace>
        <oboInOwl:id>GAZ:00123810</oboInOwl:id>
        <rdfs:label>Habro Woreda</rdfs:label>
    </owl:NamedIndividual>
    


    <!-- http://purl.obolibrary.org/obo/GAZ_00123811 -->

    <owl:NamedIndividual rdf:about="http://purl.obolibrary.org/obo/GAZ_00123811">
        <obo:RO_0001025 rdf:resource="http://purl.obolibrary.org/obo/GAZ_00031124"/>
        <obo:IAO_0000115>One of the 180 woredas in the Oromia Region of Ethiopia. Located in the Mirab Hararghe Zone, Guba Koricha, according to the OCHA map (2005) is bordered on the south by Darolebu, on the southwest by the Arsi Zone, on the west by the Afar Region, on the north by Mieso, on the northeast by Chiro, on the east by Habro, and on the southeast by Boke. Towns in Guba Koricha include Bedey, Chemeleleka and Kemna.</obo:IAO_0000115>
        <oboInOwl:hasOBONamespace>GAZ</oboInOwl:hasOBONamespace>
        <oboInOwl:id>GAZ:00123811</oboInOwl:id>
        <rdfs:label>Guba Koricha Woreda</rdfs:label>
    </owl:NamedIndividual>
    


    <!-- http://purl.obolibrary.org/obo/GAZ_00123812 -->

    <owl:NamedIndividual rdf:about="http://purl.obolibrary.org/obo/GAZ_00123812">
        <obo:RO_0001025 rdf:resource="http://purl.obolibrary.org/obo/GAZ_00031124"/>
        <obo:IAO_0000115>One of the 180 woredas in the Oromia Region of Ethiopia. Part of the Mirab Hararghe Zone, Darolebu is bordered on the south by the Shebelle River which separates it from the Bale Zone, on the west by the Arsi Zone, on the northwest by Guba Koricha, on the north by the Habro, and on the east by Boke. Towns in Darolebu include Machara and Micheta.</obo:IAO_0000115>
        <oboInOwl:hasOBONamespace>GAZ</oboInOwl:hasOBONamespace>
        <oboInOwl:id>GAZ:00123812</oboInOwl:id>
        <rdfs:label>Darolebu Woreda</rdfs:label>
    </owl:NamedIndividual>
    


    <!-- http://purl.obolibrary.org/obo/GAZ_00123813 -->

    <owl:NamedIndividual rdf:about="http://purl.obolibrary.org/obo/GAZ_00123813">
        <obo:RO_0001025 rdf:resource="http://purl.obolibrary.org/obo/GAZ_00031124"/>
        <obo:IAO_0000115>One of the 180 woredas, or administrative wards, in the Oromia Region of Ethiopia. Part of the Mirab Hararghe Zone, Doba is bordered on the south by Chiro, on the west by Mieso, on the north by the Somali Region, on the east by the Misraq Hararghe Zone, and on the southeast by Tulo.</obo:IAO_0000115>
        <oboInOwl:hasOBONamespace>GAZ</oboInOwl:hasOBONamespace>
        <oboInOwl:id>GAZ:00123813</oboInOwl:id>
        <rdfs:label>Doba Woreda</rdfs:label>
    </owl:NamedIndividual>
    


    <!-- http://purl.obolibrary.org/obo/GAZ_00123814 -->

    <owl:NamedIndividual rdf:about="http://purl.obolibrary.org/obo/GAZ_00123814">
        <obo:RO_0001025 rdf:resource="http://purl.obolibrary.org/obo/GAZ_00031124"/>
        <obo:IAO_0000115>One of the 180 woredas in the Oromia Region of Ethiopia. Part of the Mirab Hararghe Zone, Chiro is bordered on the south by Kuni, on the west by Guba Koricha, on the northwest by Mieso, on the north by Doba, on the northeast by Tulo, and on the east by the Galetti River which separates it from Mesela and the Misraq Hararghe Zone. Towns in Chiro include Asebe Teferi and Kuni.</obo:IAO_0000115>
        <oboInOwl:hasOBONamespace>GAZ</oboInOwl:hasOBONamespace>
        <oboInOwl:id>GAZ:00123814</oboInOwl:id>
        <rdfs:label>Chiro Woreda</rdfs:label>
    </owl:NamedIndividual>
    


    <!-- http://purl.obolibrary.org/obo/GAZ_00123815 -->

    <owl:NamedIndividual rdf:about="http://purl.obolibrary.org/obo/GAZ_00123815">
        <obo:RO_0001025 rdf:resource="http://purl.obolibrary.org/obo/GAZ_00031125"/>
        <obo:IAO_0000115>One of the 180 woredas in the Oromia Region of Ethiopia. Part of the Mirab Shewa Zone, Adda Berga is bordered on the south by Walmara, on the southwest by Ejerie, on the west by Meta Robi, and on the north and east by the Muger River which separates it from the Semien Shewa Zone. Towns in Adda Berga include Enchini, Muger and Reji.</obo:IAO_0000115>
        <oboInOwl:hasOBONamespace>GAZ</oboInOwl:hasOBONamespace>
        <oboInOwl:id>GAZ:00123815</oboInOwl:id>
        <rdfs:label>Adda Berga Woreda</rdfs:label>
    </owl:NamedIndividual>
    


    <!-- http://purl.obolibrary.org/obo/GAZ_00123816 -->

    <owl:NamedIndividual rdf:about="http://purl.obolibrary.org/obo/GAZ_00123816">
        <obo:RO_0001025 rdf:resource="http://purl.obolibrary.org/obo/GAZ_00031125"/>
        <obo:IAO_0000115>One of the 180 woredas in the Oromia Region of Ethiopia. Part of the Mirab Shewa Zone, Jedlu is bordered on the south by Dendi, on the southwest by Ambo, on the north by Ginde Beret, on the northeast by Meta Robi, and on the southeast by Ejerie. Towns in Jedlu include Chebi, Gojo and Shekute.</obo:IAO_0000115>
        <oboInOwl:hasOBONamespace>GAZ</oboInOwl:hasOBONamespace>
        <oboInOwl:id>GAZ:00123816</oboInOwl:id>
        <rdfs:label>Jeldu Woreda</rdfs:label>
    </owl:NamedIndividual>
    


    <!-- http://purl.obolibrary.org/obo/GAZ_00123817 -->

    <owl:NamedIndividual rdf:about="http://purl.obolibrary.org/obo/GAZ_00123817">
        <obo:RO_0001025 rdf:resource="http://purl.obolibrary.org/obo/GAZ_00031125"/>
        <obo:IAO_0000115>One of the 180 woredas in the Oromia Region of Ethiopia. Part of the Mirab Shewa Zone, Cheliya is bordered on the south by Nono and Dano, on the southwest by the Jimma Zone, on the west by Bako Tibe, on the northwest by the Guder River which separates it from the Mirab Welega Zone, on the north by Ginde Beret, on the northeast by Jeldu, on the east by Ambo, and on the southeast by Tikur. Towns in Cheliya include Babiche, Ejaji, Gedo and Hamus Gebeya.</obo:IAO_0000115>
        <oboInOwl:hasOBONamespace>GAZ</oboInOwl:hasOBONamespace>
        <oboInOwl:id>GAZ:00123817</oboInOwl:id>
        <rdfs:label>Cheliya Woreda</rdfs:label>
    </owl:NamedIndividual>
    


    <!-- http://purl.obolibrary.org/obo/GAZ_00123818 -->

    <owl:NamedIndividual rdf:about="http://purl.obolibrary.org/obo/GAZ_00123818">
        <obo:RO_0001025 rdf:resource="http://purl.obolibrary.org/obo/GAZ_00031125"/>
        <obo:IAO_0000115>One of the 180 woredas in the Oromia Region of Ethiopia. Part of the Mirab Shewa Zone, Nono is bordered on the southwest by the Gibe River which separates it from the Jimma Zone, on the northwest by Dano, on the north by Cheliya, on the northeast by Tikur, on the east by Amaya, and on the southeast by the Southern Nations, Nationalities and Peoples Region. The major town in Nono is Shanan.</obo:IAO_0000115>
        <oboInOwl:hasOBONamespace>GAZ</oboInOwl:hasOBONamespace>
        <oboInOwl:id>GAZ:00123818</oboInOwl:id>
        <rdfs:label>Nono Woreda</rdfs:label>
    </owl:NamedIndividual>
    


    <!-- http://purl.obolibrary.org/obo/GAZ_00123819 -->

    <owl:NamedIndividual rdf:about="http://purl.obolibrary.org/obo/GAZ_00123819">
        <obo:RO_0001025 rdf:resource="http://purl.obolibrary.org/obo/GAZ_00031125"/>
        <obo:IAO_0000115>One of the 180 woredas in the Oromia Region of Ethiopia. Part of the Mirab Shewa Zone, Tikur is bordered on the southwest by Nono, on the northwest by Cheliya, on the northeast by Ambo, and on the southeast by Amaya. The major town in Tikur is Tikur Enchini.</obo:IAO_0000115>
        <oboInOwl:hasOBONamespace>GAZ</oboInOwl:hasOBONamespace>
        <oboInOwl:id>GAZ:00123819</oboInOwl:id>
        <rdfs:label>Tikur Woreda</rdfs:label>
    </owl:NamedIndividual>
    


    <!-- http://purl.obolibrary.org/obo/GAZ_00123820 -->

    <owl:NamedIndividual rdf:about="http://purl.obolibrary.org/obo/GAZ_00123820">
        <obo:RO_0001025 rdf:resource="http://purl.obolibrary.org/obo/GAZ_00031125"/>
        <obo:IAO_0000115>One of the 180 woredas in the Oromia Region of Ethiopia. Part of the Mirab Shewa Zone, Walisona Goro is bordered on the south by the Southern Nations, Nationalities and Peoples Region, on the west by Amaya, on the northwest by Wonchi, on the north by Dawo, on the northeast by Becho and on the east by Kokir. Towns in Walisona Goro include Dilala, Goro, Gurura and Waliso.</obo:IAO_0000115>
        <oboInOwl:hasOBONamespace>GAZ</oboInOwl:hasOBONamespace>
        <oboInOwl:id>GAZ:00123820</oboInOwl:id>
        <rdfs:label>Walisona Goro Woreda</rdfs:label>
    </owl:NamedIndividual>
    


    <!-- http://purl.obolibrary.org/obo/GAZ_00123821 -->

    <owl:NamedIndividual rdf:about="http://purl.obolibrary.org/obo/GAZ_00123821">
        <obo:RO_0001025 rdf:resource="http://purl.obolibrary.org/obo/GAZ_00031125"/>
        <obo:IAO_0000115>One of the 180 woredas in the Oromia Region of Ethiopia. Part of the Mirab Shewa Zone, Kokir is bordered on the south by the Southern Nations, Nationalities and Peoples Region, on the west by Walisona Goro, on the north by Becho, on the northeast by Tole, and on the east by Kersana Kondaltiti. The major town in Kokir is Harbu Chulule.</obo:IAO_0000115>
        <oboInOwl:hasOBONamespace>GAZ</oboInOwl:hasOBONamespace>
        <oboInOwl:id>GAZ:00123821</oboInOwl:id>
        <rdfs:label>Kokir Woreda</rdfs:label>
    </owl:NamedIndividual>
    


    <!-- http://purl.obolibrary.org/obo/GAZ_00123822 -->

    <owl:NamedIndividual rdf:about="http://purl.obolibrary.org/obo/GAZ_00123822">
        <obo:RO_0001025 rdf:resource="http://purl.obolibrary.org/obo/GAZ_00031125"/>
        <obo:IAO_0000115>One of the 180 woredas in the Oromia Region of Ethiopia. Part of the Mirab Shewa Zone, Ejerie is bordered on the south by Elu, on the west by Dendi, on the northwest by Jeldu, on the north by Meta Robi, on the northeast by Adda Berga, on the east by Walmara, and on the southeast by Alem Gena. The major town in Ejerie is Addis Alem; this woreda is sometimes referred to by the name of this town.</obo:IAO_0000115>
        <oboInOwl:hasOBONamespace>GAZ</oboInOwl:hasOBONamespace>
        <oboInOwl:id>GAZ:00123822</oboInOwl:id>
        <rdfs:label>Ejerie Woreda</rdfs:label>
    </owl:NamedIndividual>
    


    <!-- http://purl.obolibrary.org/obo/GAZ_00123823 -->

    <owl:NamedIndividual rdf:about="http://purl.obolibrary.org/obo/GAZ_00123823">
        <obo:RO_0001025 rdf:resource="http://purl.obolibrary.org/obo/GAZ_00031125"/>
        <obo:IAO_0000115>One of the 180 woredas in the Oromia Region of Ethiopia. Part of the Mirab Shewa Zone, Tole is bordered on the southwest by Kokir, on the west by Becho, on the northwest by Elu, on the northeast by Alem Gena, and on the east and south by Kersana Kondaltiti. The major town in Tole is Bentu Liben.</obo:IAO_0000115>
        <oboInOwl:hasOBONamespace>GAZ</oboInOwl:hasOBONamespace>
        <oboInOwl:id>GAZ:00123823</oboInOwl:id>
        <rdfs:label>Tole Woreda</rdfs:label>
    </owl:NamedIndividual>
    


    <!-- http://purl.obolibrary.org/obo/GAZ_00123824 -->

    <owl:NamedIndividual rdf:about="http://purl.obolibrary.org/obo/GAZ_00123824">
        <obo:RO_0001025 rdf:resource="http://purl.obolibrary.org/obo/GAZ_00031125"/>
        <obo:IAO_0000115>One of the 180 woredas in the Oromia Region of Ethiopia. Part of the Mirab Shewa Zone, Walmara is bordered on the south by Alem Gena, on the west by Ejerie, on the north by Adda Berga, on the northeast by the Semien Shewa Zone, and on the east by the city of Addis Ababa. Towns in Walmara include Burayu, Holeta Genet and Menagesha Kolobo.</obo:IAO_0000115>
        <oboInOwl:hasOBONamespace>GAZ</oboInOwl:hasOBONamespace>
        <oboInOwl:id>GAZ:00123824</oboInOwl:id>
        <rdfs:label>Walmara Woreda</rdfs:label>
    </owl:NamedIndividual>
    


    <!-- http://purl.obolibrary.org/obo/GAZ_00123825 -->

    <owl:NamedIndividual rdf:about="http://purl.obolibrary.org/obo/GAZ_00123825">
        <obo:RO_0001025 rdf:resource="http://purl.obolibrary.org/obo/GAZ_00031125"/>
        <obo:IAO_0000115>One of the 180 woredas in the Oromia Region of Ethiopia. Part of the Mirab Shewa Zone, Kersana Kondaltiti is bordered on the south by the Southern Nations, Nationalities and Peoples Region, on the west by Kokir, on the northwest by Tole, on the northeast by Alem Gena, and on the east by the Misraq Shewa Zone. The major town in Kersana Kondaltiti is Leman.</obo:IAO_0000115>
        <oboInOwl:hasOBONamespace>GAZ</oboInOwl:hasOBONamespace>
        <oboInOwl:id>GAZ:00123825</oboInOwl:id>
        <rdfs:label>Kersana Kondaltiti Woreda</rdfs:label>
    </owl:NamedIndividual>
    


    <!-- http://purl.obolibrary.org/obo/GAZ_00123826 -->

    <owl:NamedIndividual rdf:about="http://purl.obolibrary.org/obo/GAZ_00123826">
        <obo:RO_0001025 rdf:resource="http://purl.obolibrary.org/obo/GAZ_00031125"/>
        <obo:IAO_0000115>One of the 180 woredas in the Oromia Region of Ethiopia. Part of the Mirab Shewa Zone, Meta Robi is bordered on the south by Ejerie, on the southwest by Jeldu, on the northwest by Ginde Beret, on the north by the Muger River which separates it from the Semien Shewa Zone, and on the east by Adda Berga. The major town in Meta Robi is Sheno.</obo:IAO_0000115>
        <oboInOwl:hasOBONamespace>GAZ</oboInOwl:hasOBONamespace>
        <oboInOwl:id>GAZ:00123826</oboInOwl:id>
        <rdfs:label>Meta Robi Woreda</rdfs:label>
    </owl:NamedIndividual>
    


    <!-- http://purl.obolibrary.org/obo/GAZ_00123827 -->

    <owl:NamedIndividual rdf:about="http://purl.obolibrary.org/obo/GAZ_00123827">
        <obo:RO_0001025 rdf:resource="http://purl.obolibrary.org/obo/GAZ_00031125"/>
        <obo:IAO_0000115>One of the 180 woredas in the Oromia Region of Ethiopia. Part of the Debub Mirab Shewa Zone, Dawo is bordered on the southwest by Waliso, on the west and north by Dendi, on the east by Elu, and on the southeast by Becho. The major town in Dawo is Busa.</obo:IAO_0000115>
        <oboInOwl:hasOBONamespace>GAZ</oboInOwl:hasOBONamespace>
        <oboInOwl:id>GAZ:00123827</oboInOwl:id>
        <rdfs:label>Dawo Woreda</rdfs:label>
    </owl:NamedIndividual>
    


    <!-- http://purl.obolibrary.org/obo/GAZ_00123828 -->

    <owl:NamedIndividual rdf:about="http://purl.obolibrary.org/obo/GAZ_00123828">
        <obo:RO_0001025 rdf:resource="http://purl.obolibrary.org/obo/GAZ_00031125"/>
        <obo:IAO_0000115>One of the 180 woredas in the Oromia Region of Ethiopia. Part of the Mirab Shewa Zone, Amaya is bordered on the south by the Southern Nations, Nationalities and Peoples Region, on the west by Nono, on the northwest by Tikur, on the northeast by Wonchi, and on the east by Walisona Goro. The major town in Amaya is Gindo.</obo:IAO_0000115>
        <oboInOwl:hasOBONamespace>GAZ</oboInOwl:hasOBONamespace>
        <oboInOwl:id>GAZ:00123828</oboInOwl:id>
        <rdfs:label>Amaya Woreda</rdfs:label>
    </owl:NamedIndividual>
    


    <!-- http://purl.obolibrary.org/obo/GAZ_00123829 -->

    <owl:NamedIndividual rdf:about="http://purl.obolibrary.org/obo/GAZ_00123829">
        <obo:RO_0001025 rdf:resource="http://purl.obolibrary.org/obo/GAZ_00031125"/>
        <obo:IAO_0000115>One of the 180 woredas, or districts, in the Oromia Region of Ethiopia. Part of the Mirab Shewa Zone, Bako Tibe is bordered on the south, west and north by the Misraq Welega Zone, and on the east by Cheliya. Towns in Bako Tibe include Bako, Tibe and Shoboka.</obo:IAO_0000115>
        <oboInOwl:hasOBONamespace>GAZ</oboInOwl:hasOBONamespace>
        <oboInOwl:id>GAZ:00123829</oboInOwl:id>
        <rdfs:label>Bako Tibe Woreda</rdfs:label>
    </owl:NamedIndividual>
    


    <!-- http://purl.obolibrary.org/obo/GAZ_00123830 -->

    <owl:NamedIndividual rdf:about="http://purl.obolibrary.org/obo/GAZ_00123830">
        <obo:RO_0001025 rdf:resource="http://purl.obolibrary.org/obo/GAZ_00031125"/>
        <obo:IAO_0000115>One of the 180 woredas in the Oromia Region of Ethiopia. Part of the Mirab Shewa Zone, Alem Gena is bordered on the south by Kersana Kondaltiti, on the southwest by Tole, on the west by Elu, on the northwest by Ejerie, on the north by Walmara, on the northeast by the city of Addis Ababa, and on the southeast by the Misraq Shewa Zone. Other towns in Alem Gena include Awash Kunture, Sebeta, and Tefki.</obo:IAO_0000115>
        <oboInOwl:hasOBONamespace>GAZ</oboInOwl:hasOBONamespace>
        <oboInOwl:id>GAZ:00123830</oboInOwl:id>
        <rdfs:label>Alem Gena Woreda</rdfs:label>
    </owl:NamedIndividual>
    


    <!-- http://purl.obolibrary.org/obo/GAZ_00123831 -->

    <owl:NamedIndividual rdf:about="http://purl.obolibrary.org/obo/GAZ_00123831">
        <obo:RO_0001025 rdf:resource="http://purl.obolibrary.org/obo/GAZ_00031125"/>
        <obo:IAO_0000115>One of the 180 woredas in the Oromia Region of Ethiopia. Part of the Mirab Shewa Zone, Elu is bordered on the south by Becho, on the west by Dawo, on the northwest by Dendi, on the northeast by Ejerie, and on the east by Alem Gena. Towns in Elu include Asgori and Teji.</obo:IAO_0000115>
        <oboInOwl:hasOBONamespace>GAZ</oboInOwl:hasOBONamespace>
        <oboInOwl:id>GAZ:00123831</oboInOwl:id>
        <rdfs:label>Elu Woreda</rdfs:label>
    </owl:NamedIndividual>
    


    <!-- http://purl.obolibrary.org/obo/GAZ_00123832 -->

    <owl:NamedIndividual rdf:about="http://purl.obolibrary.org/obo/GAZ_00123832">
        <obo:RO_0001025 rdf:resource="http://purl.obolibrary.org/obo/GAZ_00031125"/>
        <obo:IAO_0000115>One of the 180 woredas in the Oromia Region of Ethiopia. Part of the Mirab Shewa Zone, Wonchi is bordered on the southwest by Amaya, on the northwest by Ambo, on the northeast by Dendi, and on the southeast by Walisona Goro. The major town in Wonchi is Chitu.</obo:IAO_0000115>
        <oboInOwl:hasOBONamespace>GAZ</oboInOwl:hasOBONamespace>
        <oboInOwl:id>GAZ:00123832</oboInOwl:id>
        <rdfs:label>Wonchi Woreda</rdfs:label>
    </owl:NamedIndividual>
    


    <!-- http://purl.obolibrary.org/obo/GAZ_00123833 -->

    <owl:NamedIndividual rdf:about="http://purl.obolibrary.org/obo/GAZ_00123833">
        <obo:RO_0001025 rdf:resource="http://purl.obolibrary.org/obo/GAZ_00031125"/>
        <obo:IAO_0000115>One of the 180 woredas in the Oromia Region of Ethiopia. Part of the Mirab Shewa Zone, Becho is bordered on the south by Kokir, on the west by Walisona Goro, on the northwest by Dawo, on the north by Elu, and on the east by Tole. The major town in Becho is Tulu Bolo.</obo:IAO_0000115>
        <oboInOwl:hasOBONamespace>GAZ</oboInOwl:hasOBONamespace>
        <oboInOwl:id>GAZ:00123833</oboInOwl:id>
        <rdfs:label>Becho Woreda</rdfs:label>
    </owl:NamedIndividual>
    


    <!-- http://purl.obolibrary.org/obo/GAZ_00123834 -->

    <owl:NamedIndividual rdf:about="http://purl.obolibrary.org/obo/GAZ_00123834">
        <obo:RO_0001025 rdf:resource="http://purl.obolibrary.org/obo/GAZ_00031125"/>
        <obo:IAO_0000115>One of the 180 woredas in the Oromia Region of Ethiopia. Part of the Mirab Shewa Zone, Dendi is bordered on the south by Wonchi, on the west by Ambo, on the north by Jeldu, on the east by Ejerie, and on the southeast by Dawo. Towns in Dendi include Ehud Gebeya, Ginchi and Olonkomi.</obo:IAO_0000115>
        <oboInOwl:hasOBONamespace>GAZ</oboInOwl:hasOBONamespace>
        <oboInOwl:id>GAZ:00123834</oboInOwl:id>
        <rdfs:label>Dendi Woreda</rdfs:label>
    </owl:NamedIndividual>
    


    <!-- http://purl.obolibrary.org/obo/GAZ_00123835 -->

    <owl:NamedIndividual rdf:about="http://purl.obolibrary.org/obo/GAZ_00123835">
        <obo:RO_0001025 rdf:resource="http://purl.obolibrary.org/obo/GAZ_00031125"/>
        <obo:IAO_0000115>One of the 180 woredas in the Oromia Region of Ethiopia. Part of the Mirab Shewa Zone, Dano is bordered on the southwest by the Jimma Zone, on the north by Cheliya, and on the southeast by Nono; part of the boundary with the Jimma Zone is defined by the Gibe River. The major town in Dano is Sayo.</obo:IAO_0000115>
        <oboInOwl:hasOBONamespace>GAZ</oboInOwl:hasOBONamespace>
        <oboInOwl:id>GAZ:00123835</oboInOwl:id>
        <rdfs:label>Dano Woreda</rdfs:label>
    </owl:NamedIndividual>
    


    <!-- http://purl.obolibrary.org/obo/GAZ_00123836 -->

    <owl:NamedIndividual rdf:about="http://purl.obolibrary.org/obo/GAZ_00123836">
        <obo:RO_0001025 rdf:resource="http://purl.obolibrary.org/obo/GAZ_00123874"/>
        <obo:IAO_0000115>A lake.</obo:IAO_0000115>
        <oboInOwl:hasOBONamespace>GAZ</oboInOwl:hasOBONamespace>
        <oboInOwl:id>GAZ:00123836</oboInOwl:id>
        <rdfs:label>Lake Basaka</rdfs:label>
    </owl:NamedIndividual>
    


    <!-- http://purl.obolibrary.org/obo/GAZ_00123837 -->

    <owl:NamedIndividual rdf:about="http://purl.obolibrary.org/obo/GAZ_00123837">
        <obo:RO_0001025 rdf:resource="http://purl.obolibrary.org/obo/GAZ_00031121"/>
        <obo:IAO_0000115>One of the 180 woredas in the Oromia Region of Ethiopia. Part of the Mirab Welega Zone, Anfillo is bordered on the southwest by the Gambela Region, on the north by Jimma Gidami, on the northeast by Hawa Welele, and on the east by Sayo. The major town in Anfillo is Mugi.</obo:IAO_0000115>
        <oboInOwl:hasOBONamespace>GAZ</oboInOwl:hasOBONamespace>
        <oboInOwl:id>GAZ:00123837</oboInOwl:id>
        <rdfs:label>Anfillo Woreda</rdfs:label>
    </owl:NamedIndividual>
    


    <!-- http://purl.obolibrary.org/obo/GAZ_00123838 -->

    <owl:NamedIndividual rdf:about="http://purl.obolibrary.org/obo/GAZ_00123838">
        <obo:RO_0001025 rdf:resource="http://purl.obolibrary.org/obo/GAZ_00031121"/>
        <obo:IAO_0000115>One of the 180 woredas in the Oromia Region of Ethiopia. Part of the Mirab Welega Zone, Mana Sibu is bordered on the south by Jarso, on the southwest by Begi, on the north by the Benishangul-Gumuz Region, and on the southeast by Nejo. Mendi is the administrative center; other towns in Mana Sibu include Kiltu Kara.</obo:IAO_0000115>
        <oboInOwl:hasOBONamespace>GAZ</oboInOwl:hasOBONamespace>
        <oboInOwl:id>GAZ:00123838</oboInOwl:id>
        <rdfs:label>Mana Sibu Woreda</rdfs:label>
    </owl:NamedIndividual>
    


    <!-- http://purl.obolibrary.org/obo/GAZ_00123839 -->

    <owl:NamedIndividual rdf:about="http://purl.obolibrary.org/obo/GAZ_00123839">
        <obo:RO_0001025 rdf:resource="http://purl.obolibrary.org/obo/GAZ_00031121"/>
        <obo:IAO_0000115>One of the 180 woredas in the Oromia Region of Ethiopia. Part of the Mirab Welega Zone, Nole Kaba is bordered on the south by the Illubabor Zone, on the west by Dale Lalo, on the northwest by Yubdo, and on the northeast by Haru. Towns in Nole Kaba include Bube and Debeso.</obo:IAO_0000115>
        <oboInOwl:hasOBONamespace>GAZ</oboInOwl:hasOBONamespace>
        <oboInOwl:id>GAZ:00123839</oboInOwl:id>
        <rdfs:label>Nole Kaba Woreda</rdfs:label>
    </owl:NamedIndividual>
    


    <!-- http://purl.obolibrary.org/obo/GAZ_00123840 -->

    <owl:NamedIndividual rdf:about="http://purl.obolibrary.org/obo/GAZ_00123840">
        <obo:RO_0001025 rdf:resource="http://purl.obolibrary.org/obo/GAZ_00031121"/>
        <obo:IAO_0000115>One of the 180 woredas in the Oromia Region of Ethiopia. Part of the Mirab Welega Zone, Begi is bordered on the south by Jimma Gidami, on the west and north by the Benishangul-Gumuz Region, on the northeast by Mana Sibu, on the east by Jarso, and on the southeast by Gawo Dale. Towns in Begi include Begi, Kober and Segno Gebeya.</obo:IAO_0000115>
        <oboInOwl:hasOBONamespace>GAZ</oboInOwl:hasOBONamespace>
        <oboInOwl:id>GAZ:00123840</oboInOwl:id>
        <rdfs:label>Begi Woreda</rdfs:label>
    </owl:NamedIndividual>
    


    <!-- http://purl.obolibrary.org/obo/GAZ_00123841 -->

    <owl:NamedIndividual rdf:about="http://purl.obolibrary.org/obo/GAZ_00123841">
        <obo:RO_0001025 rdf:resource="http://purl.obolibrary.org/obo/GAZ_00031121"/>
        <obo:IAO_0000115>One of the 180 woredas in the Oromia Region of Ethiopia. Part of the Mirab Welega Zone, Sayo is bordered on the south by the Gambela Region, on the west by Anfillo, on the north by Hawa Welele, and on the east by the Birbir River which separates it from the Illubabor Zone.</obo:IAO_0000115>
        <oboInOwl:hasOBONamespace>GAZ</oboInOwl:hasOBONamespace>
        <oboInOwl:id>GAZ:00123841</oboInOwl:id>
        <rdfs:label>Sayo Woreda</rdfs:label>
    </owl:NamedIndividual>
    


    <!-- http://purl.obolibrary.org/obo/GAZ_00123842 -->

    <owl:NamedIndividual rdf:about="http://purl.obolibrary.org/obo/GAZ_00123842">
        <obo:RO_0001025 rdf:resource="http://purl.obolibrary.org/obo/GAZ_00031121"/>
        <obo:IAO_0000115>One of the 180 woredas in the Oromia Region of Ethiopia. Part of the Mirab Welega Zone, Gawo Dale is bordered on the south by Hawa Welele, on the west by Jimma Gidami, on the northwest by Begi, on the north by Jarso, on the northeast by Ayra Guliso, on the east by Dale Lalo, and on the southeast by the Illubabor Zone. Towns in Gawo Dale include Chanka and Kake.</obo:IAO_0000115>
        <oboInOwl:hasOBONamespace>GAZ</oboInOwl:hasOBONamespace>
        <oboInOwl:id>GAZ:00123842</oboInOwl:id>
        <rdfs:label>Gawo Dale Woreda</rdfs:label>
    </owl:NamedIndividual>
    


    <!-- http://purl.obolibrary.org/obo/GAZ_00123843 -->

    <owl:NamedIndividual rdf:about="http://purl.obolibrary.org/obo/GAZ_00123843">
        <obo:RO_0001025 rdf:resource="http://purl.obolibrary.org/obo/GAZ_00031121"/>
        <obo:IAO_0000115>One of the 180 woredas in the Oromia Region of Ethiopia. Part of the Mirab Welega Zone, Nejo is bordered on the southeast by Boji, on the west by Jarso, on the northwest by Mana Sibu, and on the north and east by the Benishangul-Gumuz Region. Towns in Nejo include Gori, Nejo and Wara Jiru.</obo:IAO_0000115>
        <oboInOwl:hasOBONamespace>GAZ</oboInOwl:hasOBONamespace>
        <oboInOwl:id>GAZ:00123843</oboInOwl:id>
        <rdfs:label>Nejo Woreda</rdfs:label>
    </owl:NamedIndividual>
    


    <!-- http://purl.obolibrary.org/obo/GAZ_00123844 -->

    <owl:NamedIndividual rdf:about="http://purl.obolibrary.org/obo/GAZ_00123844">
        <obo:RO_0001025 rdf:resource="http://purl.obolibrary.org/obo/GAZ_00031121"/>
        <obo:IAO_0000115>One of the 180 woredas in the Oromia Region of Ethiopia. Part of the Mirab Welega Zone, Haru is bordered on the south by Nole Kaba, on the southwest by Dale Lalo, on the west by Yubdo, on the north by Gimbi, on the east by an exclave of the Benishangul-Gumuz Region, and on the southeast by the Illubabor Zone. Towns in Haru include Guyi and Guyu Abo.</obo:IAO_0000115>
        <oboInOwl:hasOBONamespace>GAZ</oboInOwl:hasOBONamespace>
        <oboInOwl:id>GAZ:00123844</oboInOwl:id>
        <rdfs:label>Haru Woreda</rdfs:label>
    </owl:NamedIndividual>
    


    <!-- http://purl.obolibrary.org/obo/GAZ_00123845 -->

    <owl:NamedIndividual rdf:about="http://purl.obolibrary.org/obo/GAZ_00123845">
        <obo:RO_0001025 rdf:resource="http://purl.obolibrary.org/obo/GAZ_00031121"/>
        <obo:IAO_0000115>One of the 180 woredas in the Oromia Region of Ethiopia. Part of the Mirab Welega Zone, Lalo Asabi is bordered on the south by Yubdo, on the west by Ayra Guliso, on the north by Boji, on the east by the Benishangul-Gumuz Region, and on the southeast by Gimbi. Towns in Lalo Asabi include Dongoro and Inango.</obo:IAO_0000115>
        <oboInOwl:hasOBONamespace>GAZ</oboInOwl:hasOBONamespace>
        <oboInOwl:id>GAZ:00123845</oboInOwl:id>
        <rdfs:label>Lalo Asabi Woreda</rdfs:label>
    </owl:NamedIndividual>
    


    <!-- http://purl.obolibrary.org/obo/GAZ_00123846 -->

    <owl:NamedIndividual rdf:about="http://purl.obolibrary.org/obo/GAZ_00123846">
        <obo:RO_0001025 rdf:resource="http://purl.obolibrary.org/obo/GAZ_00031121"/>
        <obo:IAO_0000115>One of the 180 woredas in the Oromia Region of Ethiopia. Part of the Mirab Welega Zone, Jarso is bordered on the south by Ayra Guliso, on the southwest by Gawo Dale, on the west by Begi, on the north by Mana Sibu, on the northeast by Nejo, and on the southeast by Boji. Towns in Jarso include Dabeka and Geba Dafino.</obo:IAO_0000115>
        <oboInOwl:hasOBONamespace>GAZ</oboInOwl:hasOBONamespace>
        <oboInOwl:id>GAZ:00123846</oboInOwl:id>
        <rdfs:label>Jarso Woreda</rdfs:label>
    </owl:NamedIndividual>
    


    <!-- http://purl.obolibrary.org/obo/GAZ_00123847 -->

    <owl:NamedIndividual rdf:about="http://purl.obolibrary.org/obo/GAZ_00123847">
        <obo:RO_0001025 rdf:resource="http://purl.obolibrary.org/obo/GAZ_00031121"/>
        <obo:IAO_0000115>One of the 180 woredas in the Oromia Region of Ethiopia. Part of the Mirab Welega Zone, Jimma Gidami is bordered on the south by Anfillo, on the west by Sudan, on the northwest by the Benishangul-Gumuz Region, on the north by Begi, on the east by Gawo Dale, and on the east by Hawa Welele. Towns in Jimma Gidami include Gidami and Nunu.</obo:IAO_0000115>
        <oboInOwl:hasOBONamespace>GAZ</oboInOwl:hasOBONamespace>
        <oboInOwl:id>GAZ:00123847</oboInOwl:id>
        <rdfs:label>Jimma Gidami Woreda</rdfs:label>
    </owl:NamedIndividual>
    


    <!-- http://purl.obolibrary.org/obo/GAZ_00123848 -->

    <owl:NamedIndividual rdf:about="http://purl.obolibrary.org/obo/GAZ_00123848">
        <obo:RO_0001025 rdf:resource="http://purl.obolibrary.org/obo/GAZ_00031121"/>
        <obo:IAO_0000115>One of the 180 woredas in the Oromia Region of Ethiopia. Part of the Mirab Welega Zone, Hawa Welele is bordered on the south by Sayo, on the west by Anfillo, on the northwest by Jimma Gidami, on the north and east by Gawo Dale, and on the southeast by the Illubabor Zone. Towns in Hawa Welele include Rob Gebeya and Tejo.</obo:IAO_0000115>
        <oboInOwl:hasOBONamespace>GAZ</oboInOwl:hasOBONamespace>
        <oboInOwl:id>GAZ:00123848</oboInOwl:id>
        <rdfs:label>Hawa Welele Woreda</rdfs:label>
    </owl:NamedIndividual>
    


    <!-- http://purl.obolibrary.org/obo/GAZ_00123849 -->

    <owl:NamedIndividual rdf:about="http://purl.obolibrary.org/obo/GAZ_00123849">
        <obo:RO_0001025 rdf:resource="http://purl.obolibrary.org/obo/GAZ_00031121"/>
        <obo:IAO_0000115>One of the 180 woredas in the Oromia Region of Ethiopia. Part of the Mirab Welega Zone, Yubdo is bordered on the south by Nole Kaba, on the west by Dale Lalo, on the northwest by Ayra Guliso, on the northeast by Lalo Asabi, on the east by Gimbi, and on the southeast by Haru. Towns in Yubdo include Ganji and Yubdo.</obo:IAO_0000115>
        <oboInOwl:hasOBONamespace>GAZ</oboInOwl:hasOBONamespace>
        <oboInOwl:id>GAZ:00123849</oboInOwl:id>
        <rdfs:label>Yubdo Woreda</rdfs:label>
    </owl:NamedIndividual>
    


    <!-- http://purl.obolibrary.org/obo/GAZ_00123850 -->

    <owl:NamedIndividual rdf:about="http://purl.obolibrary.org/obo/GAZ_00123850">
        <obo:RO_0001025 rdf:resource="http://purl.obolibrary.org/obo/GAZ_00031121"/>
        <obo:IAO_0000115>One of the 180 woredas in the Oromia Region of Ethiopia. Part of the Mirab Welega Zone, Dale Lalo is bordered on the south by the Illubabor Zone, on the west by Gawo Dale, on the north by Ayra Guliso, on the northeast by Yubdo, and on the east by Nole Kaba. Towns in Dale Lalo include Alem and Teferi.</obo:IAO_0000115>
        <oboInOwl:hasOBONamespace>GAZ</oboInOwl:hasOBONamespace>
        <oboInOwl:id>GAZ:00123850</oboInOwl:id>
        <rdfs:label>Dale Lalo Woreda</rdfs:label>
    </owl:NamedIndividual>
    


    <!-- http://purl.obolibrary.org/obo/GAZ_00123851 -->

    <owl:NamedIndividual rdf:about="http://purl.obolibrary.org/obo/GAZ_00123851">
        <obo:RO_0001025 rdf:resource="http://purl.obolibrary.org/obo/GAZ_00031121"/>
        <obo:IAO_0000115>One of the 180 woredas in the Oromia Region of Ethiopia. Part of the Mirab Welega Zone, Gimbi is bordered on the south by Haru, on the southwest by Yubdo, on the west by Lalo Asabi, on the north by the Benishangul-Gumuz Region, on the east by the Misraq Welega Zone, and on the southeast by an exclave of the Benishangul-Gumuz Region. Towns in Gimbi include Gimbi and Homa.</obo:IAO_0000115>
        <oboInOwl:hasOBONamespace>GAZ</oboInOwl:hasOBONamespace>
        <oboInOwl:id>GAZ:00123851</oboInOwl:id>
        <rdfs:label>Gimbi Woreda</rdfs:label>
    </owl:NamedIndividual>
    


    <!-- http://purl.obolibrary.org/obo/GAZ_00123852 -->

    <owl:NamedIndividual rdf:about="http://purl.obolibrary.org/obo/GAZ_00123852">
        <obo:RO_0001025 rdf:resource="http://purl.obolibrary.org/obo/GAZ_00031121"/>
        <obo:IAO_0000115>One of the 180 woredas in the Oromia Region of Ethiopia. Part of the Mirab Welega Zone, Boji is bordered on the southwest by Ayra Guliso, on the west by Jarso, on the northwest by Nejo, on the northeast by the Benishangul-Gumuz Region, and on the southeast by Lalo Asabi. Towns in Boji include Bila and Muklemi.</obo:IAO_0000115>
        <oboInOwl:hasOBONamespace>GAZ</oboInOwl:hasOBONamespace>
        <oboInOwl:id>GAZ:00123852</oboInOwl:id>
        <rdfs:label>Boji Woreda</rdfs:label>
    </owl:NamedIndividual>
    


    <!-- http://purl.obolibrary.org/obo/GAZ_00123853 -->

    <owl:NamedIndividual rdf:about="http://purl.obolibrary.org/obo/GAZ_00123853">
        <obo:RO_0001025 rdf:resource="http://purl.obolibrary.org/obo/GAZ_00031121"/>
        <obo:IAO_0000115>One of the 180 woredas in the Oromia Region of Ethiopia. Part of the Mirab Welega Zone, Ayra Guliso is bordered on the south by Dale Lalo, on the west by Gawo Dale, on the north by Jarso, on the northeast by Boji, and on the east by Lalo Asabi. Towns in Ayra Guliso include Ayra, Cheliya Yeka and Guliso.</obo:IAO_0000115>
        <oboInOwl:hasOBONamespace>GAZ</oboInOwl:hasOBONamespace>
        <oboInOwl:id>GAZ:00123853</oboInOwl:id>
        <rdfs:label>Ayra Guliso Woreda</rdfs:label>
    </owl:NamedIndividual>
    


    <!-- http://purl.obolibrary.org/obo/GAZ_00123854 -->

    <owl:NamedIndividual rdf:about="http://purl.obolibrary.org/obo/GAZ_00123854">
        <obo:RO_0001025 rdf:resource="http://purl.obolibrary.org/obo/GAZ_00031116"/>
        <obo:IAO_0000115>One of the 180 woredas in the Oromia Region of Ethiopia. Part of the Misraq (East) Hararghe Zone, Goro Gutu is bordered on the south by Deder, on the west by the Mirab (West) Hararghe Zone, on the north by the Somali Region, and on the east by Meta. The woreda capital is Karamile; other towns include Boroda.</obo:IAO_0000115>
        <oboInOwl:hasOBONamespace>GAZ</oboInOwl:hasOBONamespace>
        <oboInOwl:id>GAZ:00123854</oboInOwl:id>
        <rdfs:label>Goro Gutu Woreda</rdfs:label>
    </owl:NamedIndividual>
    


    <!-- http://purl.obolibrary.org/obo/GAZ_00123855 -->

    <owl:NamedIndividual rdf:about="http://purl.obolibrary.org/obo/GAZ_00123855">
        <obo:RO_0001025 rdf:resource="http://purl.obolibrary.org/obo/GAZ_00031116"/>
        <obo:IAO_0000115>One of the 180 woredas in the Oromia Region of Ethiopia. Part of the Misraq (East) Hararghe Zone, Fedis is bordered on the southwest by Gola Odana Meyumuluke, on the west by Girawa, on the northwest by Haro Maya, on the north by the Harari Region, on the east by Babille, and on the southeast by the Erer River which separates it from the Somali Region. The woreda capital is Boko.</obo:IAO_0000115>
        <oboInOwl:hasOBONamespace>GAZ</oboInOwl:hasOBONamespace>
        <oboInOwl:id>GAZ:00123855</oboInOwl:id>
        <rdfs:label>Fedis Woreda</rdfs:label>
    </owl:NamedIndividual>
    


    <!-- http://purl.obolibrary.org/obo/GAZ_00123856 -->

    <owl:NamedIndividual rdf:about="http://purl.obolibrary.org/obo/GAZ_00123856">
        <obo:RO_0001025 rdf:resource="http://purl.obolibrary.org/obo/GAZ_00031116"/>
        <obo:IAO_0000115>One of the 180 woredas in the Oromia Region of Ethiopia. Part of the Misraq (East) Hararghe Zone, Kombolcha is bordered on the south by the Harari Region, on the southwest by Haro Maya, on the northwest by Dire Dawa, on the north by the Somali Region, and on the east by Jarso. The administrative center of the woreda is Melka Rafu.</obo:IAO_0000115>
        <oboInOwl:hasOBONamespace>GAZ</oboInOwl:hasOBONamespace>
        <oboInOwl:id>GAZ:00123856</oboInOwl:id>
        <rdfs:label>Kombolcha Woreda</rdfs:label>
    </owl:NamedIndividual>
    


    <!-- http://purl.obolibrary.org/obo/GAZ_00123857 -->

    <owl:NamedIndividual rdf:about="http://purl.obolibrary.org/obo/GAZ_00123857">
        <obo:RO_0001025 rdf:resource="http://purl.obolibrary.org/obo/GAZ_00031116"/>
        <obo:IAO_0000115>One of the 180 woredas in the Oromia Region of Ethiopia. Part of the Misraq (East) Hararghe Zone, Girawa is bordered on the south by Gola Odana Meyumuluke, on the west by Bedeno, on the north by Kurfa Chele, and on the east by Fedis. The woreda capital is Girawa; other towns include Megala.</obo:IAO_0000115>
        <oboInOwl:hasOBONamespace>GAZ</oboInOwl:hasOBONamespace>
        <oboInOwl:id>GAZ:00123857</oboInOwl:id>
        <rdfs:label>Girawa Woreda</rdfs:label>
    </owl:NamedIndividual>
    


    <!-- http://purl.obolibrary.org/obo/GAZ_00123858 -->

    <owl:NamedIndividual rdf:about="http://purl.obolibrary.org/obo/GAZ_00123858">
        <obo:RO_0001025 rdf:resource="http://purl.obolibrary.org/obo/GAZ_00031116"/>
        <obo:IAO_0000115>One of the 180 woredas in the Oromia Region of Ethiopia. Part of the Misraq (East) Hararghe Zone, Malka Balo is bordered on the on the west by the Mirab (West) Hararghe Zone, on the north by Deder, on the northeast by Bedeno, and on the southeast by Gola Odana Meyumuluke; part of the boundary with the Mirab Hararghe Zone is defined by the Galetti River. The woreda capital is Jaja; other towns include Harawacha and Harewa.</obo:IAO_0000115>
        <oboInOwl:hasOBONamespace>GAZ</oboInOwl:hasOBONamespace>
        <oboInOwl:id>GAZ:00123858</oboInOwl:id>
        <rdfs:label>Malka Balo Woreda</rdfs:label>
    </owl:NamedIndividual>
    


    <!-- http://purl.obolibrary.org/obo/GAZ_00123859 -->

    <owl:NamedIndividual rdf:about="http://purl.obolibrary.org/obo/GAZ_00123859">
        <obo:RO_0001025 rdf:resource="http://purl.obolibrary.org/obo/GAZ_00031116"/>
        <obo:IAO_0000115>One of the 180 woredas in the Oromia Region of Ethiopia. Part of the Misraq (East) Hararghe Zone, Jarso is bordered on the south by the Harari Region, on the west by Kombolcha, on the north by the Somali Region, and on the east by Gursum. The administrative center of this woreda is Ejersa Goro.</obo:IAO_0000115>
        <oboInOwl:hasOBONamespace>GAZ</oboInOwl:hasOBONamespace>
        <oboInOwl:id>GAZ:00123859</oboInOwl:id>
        <rdfs:label>Jarso Woreda</rdfs:label>
    </owl:NamedIndividual>
    


    <!-- http://purl.obolibrary.org/obo/GAZ_00123860 -->

    <owl:NamedIndividual rdf:about="http://purl.obolibrary.org/obo/GAZ_00123860">
        <obo:RO_0001025 rdf:resource="http://purl.obolibrary.org/obo/GAZ_00031116"/>
        <obo:IAO_0000115>One of the 180 woredas in the Oromia Region of Ethiopia. Part of the Misraq (East) Hararghe Zone, Meta is bordered on the southwest by Deder, on the northwest by Goro Gutu, on the north by the Somali Region, on the northeast by Kersa, and on the southeast by Bedeno. Towns in Meta include Chelenko and Kulubi.</obo:IAO_0000115>
        <oboInOwl:hasOBONamespace>GAZ</oboInOwl:hasOBONamespace>
        <oboInOwl:id>GAZ:00123860</oboInOwl:id>
        <rdfs:label>Meta Woreda</rdfs:label>
    </owl:NamedIndividual>
    


    <!-- http://purl.obolibrary.org/obo/GAZ_00123861 -->

    <owl:NamedIndividual rdf:about="http://purl.obolibrary.org/obo/GAZ_00123861">
        <obo:RO_0001025 rdf:resource="http://purl.obolibrary.org/obo/GAZ_00031116"/>
        <obo:IAO_0000115>One of the 180 woredas in the Oromia Region of Ethiopia. Part of the Misraq (East) Hararghe Zone, Gursum is bordered on the south by Babille, on the west by the Harari Region, on the north by Jarso, and on the east by the Somali Region. The administrative center of the woreda is Fugnan Bira.</obo:IAO_0000115>
        <oboInOwl:hasOBONamespace>GAZ</oboInOwl:hasOBONamespace>
        <oboInOwl:id>GAZ:00123861</oboInOwl:id>
        <rdfs:label>Gursum Woreda</rdfs:label>
    </owl:NamedIndividual>
    


    <!-- http://purl.obolibrary.org/obo/GAZ_00123862 -->

    <owl:NamedIndividual rdf:about="http://purl.obolibrary.org/obo/GAZ_00123862">
        <obo:RO_0001025 rdf:resource="http://purl.obolibrary.org/obo/GAZ_00031116"/>
        <obo:IAO_0000115>One of the 180 woredas in the Oromia Region of Ethiopia. Part of the Misraq (East) Hararghe Zone, Kersa is bordered on the south by Bedeno, on the west by Meta, on the north by Dire Dawa, on the northeast by Haro Maya, and on the southeast by Kurfa Chele. The woreda capital is Kersa; other towns include Lange.</obo:IAO_0000115>
        <oboInOwl:hasOBONamespace>GAZ</oboInOwl:hasOBONamespace>
        <oboInOwl:id>GAZ:00123862</oboInOwl:id>
        <rdfs:label>Kersa Woreda</rdfs:label>
    </owl:NamedIndividual>
    


    <!-- http://purl.obolibrary.org/obo/GAZ_00123863 -->

    <owl:NamedIndividual rdf:about="http://purl.obolibrary.org/obo/GAZ_00123863">
        <obo:RO_0001025 rdf:resource="http://purl.obolibrary.org/obo/GAZ_00031116"/>
        <obo:IAO_0000115>One of the 180 woredas in the Oromia Region of Ethiopia. Part of the Misraq (East) Hararghe Zone, Kurfa Chele is bordered on the south by Girawa, on the west by Bedeno, on the northwest by Kersa, and on the northeast by Haro Maya. Towns include Dawe.</obo:IAO_0000115>
        <oboInOwl:hasOBONamespace>GAZ</oboInOwl:hasOBONamespace>
        <oboInOwl:id>GAZ:00123863</oboInOwl:id>
        <rdfs:label>Kurfa Chele Woreda</rdfs:label>
    </owl:NamedIndividual>
    


    <!-- http://purl.obolibrary.org/obo/GAZ_00123864 -->

    <owl:NamedIndividual rdf:about="http://purl.obolibrary.org/obo/GAZ_00123864">
        <obo:RO_0001025 rdf:resource="http://purl.obolibrary.org/obo/GAZ_00031116"/>
        <obo:IAO_0000115>One of the 180 woredas in the Oromia Region of Ethiopia. Part of the Misraq (East) Hararghe Zone, Gola Odana Meyumuluke is bordered on the south by the Shebelle River which separates it from the Bale Zone, on the southwest by the Galetti River which separates it from the Mirab (West) Hararghe Zone, on the northwest by Malka Balo, on the north by Bedeno, on the northeast by Girawa, on the east by Fedis, and on the southeast by the Erer River which separates it from the Somali Region. The administrative center of this woreda is Burka.</obo:IAO_0000115>
        <oboInOwl:hasOBONamespace>GAZ</oboInOwl:hasOBONamespace>
        <oboInOwl:id>GAZ:00123864</oboInOwl:id>
        <rdfs:label>Gola Odana Meyumuluke Woreda</rdfs:label>
    </owl:NamedIndividual>
    


    <!-- http://purl.obolibrary.org/obo/GAZ_00123865 -->

    <owl:NamedIndividual rdf:about="http://purl.obolibrary.org/obo/GAZ_00123865">
        <obo:RO_0001025 rdf:resource="http://purl.obolibrary.org/obo/GAZ_00031119"/>
        <obo:IAO_0000115>One of the 180 woredas in the Oromia Region of Ethiopia. Part of the Misraq Shewa Zone located in the Great Rift Valley, Adami Tullu and Jido Kombolcha is bordered on the south by Arsi Negele with which it shares the shores of Lakes Abijatta and Langano, on the west by the Southern Nations, Nationalities and Peoples Region, on the north by Dugda Bora, on the northeast by Lake Zway, and on the east by the Arsi Zone. The woreda capital is Ziway; other towns include Abosa, Adami Tullu, Bulbulla, and Jido.</obo:IAO_0000115>
        <oboInOwl:hasOBONamespace>GAZ</oboInOwl:hasOBONamespace>
        <oboInOwl:id>GAZ:00123865</oboInOwl:id>
        <rdfs:label>Adami Tullu and Jido Kombolcha Woreda</rdfs:label>
    </owl:NamedIndividual>
    


    <!-- http://purl.obolibrary.org/obo/GAZ_00123866 -->

    <owl:NamedIndividual rdf:about="http://purl.obolibrary.org/obo/GAZ_00123866">
        <obo:RO_0001025 rdf:resource="http://purl.obolibrary.org/obo/GAZ_00031119"/>
        <obo:IAO_0000115>One of the 180 woredas in the Oromia Region of Ethiopia. Part of the Misraq Shewa Zone located in the Great Rift Valley, Seraro is bordered on the south and west by the Southern Nations, Nationalities and Peoples&apos; Region, on the north by Lake Shala, and on the east by Shashamene; its western boundary is defined by the course of the Bilate River. The capital of this woreda is Aje; other towns include Rope.</obo:IAO_0000115>
        <oboInOwl:hasOBONamespace>GAZ</oboInOwl:hasOBONamespace>
        <oboInOwl:id>GAZ:00123866</oboInOwl:id>
        <rdfs:label>Seraro Woreda</rdfs:label>
    </owl:NamedIndividual>
    


    <!-- http://purl.obolibrary.org/obo/GAZ_00123867 -->

    <owl:NamedIndividual rdf:about="http://purl.obolibrary.org/obo/GAZ_00123867">
        <obo:RO_0001025 rdf:resource="http://purl.obolibrary.org/obo/GAZ_00031119"/>
        <obo:IAO_0000115>One of the 180 woredas in the Oromia Region of Ethiopia. Part of the Misraq Shewa Zone located in the Great Rift Valley, Dugda Bora is bordered on the southeast by Lake Awasa, on the south by Adami Tullu and Jido Kombolcha, on the west by the Southern Nations, Nationalities and Peoples Region, on the northwest by the Mirab Shewa Zone, on the north by the Awash River which separates it from Ada&apos;a Chukala, on the northeast by Koka Reservoir which separates it from Adama, and on the east by the Arsi Zone. The administrative center of Dugda Bora is Meki; other towns include Alem Tena.</obo:IAO_0000115>
        <oboInOwl:hasOBONamespace>GAZ</oboInOwl:hasOBONamespace>
        <oboInOwl:id>GAZ:00123867</oboInOwl:id>
        <rdfs:label>Dugda Bora Woreda</rdfs:label>
    </owl:NamedIndividual>
    


    <!-- http://purl.obolibrary.org/obo/GAZ_00123868 -->

    <owl:NamedIndividual rdf:about="http://purl.obolibrary.org/obo/GAZ_00123868">
        <obo:RO_0001025 rdf:resource="http://purl.obolibrary.org/obo/GAZ_00031119"/>
        <obo:IAO_0000115>One of the 180 woredas in the Oromia Region of Ethiopia. Part of the Misraq Shewa Zone, Gimbichu is bordered on the south by Lome, on the southwest by Ada&apos;a Chukala, on the northwest by the Amhara Region, and on the east by the Afar Region. The administrative center is Chefe Donsa.</obo:IAO_0000115>
        <oboInOwl:hasOBONamespace>GAZ</oboInOwl:hasOBONamespace>
        <oboInOwl:id>GAZ:00123868</oboInOwl:id>
        <rdfs:label>Gimbichu Woreda</rdfs:label>
    </owl:NamedIndividual>
    


    <!-- http://purl.obolibrary.org/obo/GAZ_00123869 -->

    <owl:NamedIndividual rdf:about="http://purl.obolibrary.org/obo/GAZ_00123869">
        <obo:RO_0001025 rdf:resource="http://purl.obolibrary.org/obo/GAZ_00031119"/>
        <obo:IAO_0000115>One of the 180 woredas in the Oromia Region of Ethiopia. Part of the Misraq Shewa Zone, Akaki is bordered on the southwest by the Mirab Shewa Zone, on the northwest by Addis Ababa, on the north by the Semien Shewa Zone, and on the east by Ada&apos;a Chukala. The administrative center of this woreda is Dukem.</obo:IAO_0000115>
        <oboInOwl:hasOBONamespace>GAZ</oboInOwl:hasOBONamespace>
        <oboInOwl:id>GAZ:00123869</oboInOwl:id>
        <rdfs:label>Akaki Woreda</rdfs:label>
    </owl:NamedIndividual>
    


    <!-- http://purl.obolibrary.org/obo/GAZ_00123870 -->

    <owl:NamedIndividual rdf:about="http://purl.obolibrary.org/obo/GAZ_00123870">
        <obo:RO_0001025 rdf:resource="http://purl.obolibrary.org/obo/GAZ_00031119"/>
        <obo:IAO_0000115>One of the 180 woredas in the Oromia Region of Ethiopia. Part of the Misraq Shewa Zone located in the Great Rift Valley, Lome is bordered on the south by the Koka Reservoir, on the west by Ada&apos;a Chukala, on the northwest by Gimbichu, on the north by the Afar Region, and on the east by Adama. Mojo is the capital of the woreda; other towns and cities include Ejere, Ejersa and Koka.</obo:IAO_0000115>
        <oboInOwl:hasOBONamespace>GAZ</oboInOwl:hasOBONamespace>
        <oboInOwl:id>GAZ:00123870</oboInOwl:id>
        <rdfs:label>Lome Woreda</rdfs:label>
    </owl:NamedIndividual>
    


    <!-- http://purl.obolibrary.org/obo/GAZ_00123871 -->

    <owl:NamedIndividual rdf:about="http://purl.obolibrary.org/obo/GAZ_00123871">
        <obo:RO_0001025 rdf:resource="http://purl.obolibrary.org/obo/GAZ_00031119"/>
        <obo:IAO_0000115>One of the 180 woredas in the Oromia Region of Ethiopia. Part of the Misraq Shewa Zone located in the Great Rift Valley, Shashamene is bordered on the south by the Southern Nations, Nationalities and Peoples Region, on the west by Seraro, on the north by Arsi Negele, and on the east by the Arsi Zone. Towns in Shashamene include Kuyera.</obo:IAO_0000115>
        <oboInOwl:hasOBONamespace>GAZ</oboInOwl:hasOBONamespace>
        <oboInOwl:id>GAZ:00123871</oboInOwl:id>
        <rdfs:label>Shashamene Woreda</rdfs:label>
    </owl:NamedIndividual>
    


    <!-- http://purl.obolibrary.org/obo/GAZ_00123872 -->

    <owl:NamedIndividual rdf:about="http://purl.obolibrary.org/obo/GAZ_00123872">
        <obo:RO_0001025 rdf:resource="http://purl.obolibrary.org/obo/GAZ_00031119"/>
        <obo:IAO_0000115>One of the 180 woredas in the Oromia Region of Ethiopia. Part of the Misraq Shewa Zone located in the Great Rift Valley, Boset is bordered on the south by the Arsi Zone, on the west by the Awash River which separates it from Adama, on the north by the Afar Region, and on the east by Fentale. The administrative center of the woreda is Welenchiti; other towns in Boset include Bofe, Bole and Doni.</obo:IAO_0000115>
        <oboInOwl:hasOBONamespace>GAZ</oboInOwl:hasOBONamespace>
        <oboInOwl:id>GAZ:00123872</oboInOwl:id>
        <rdfs:label>Boset Woreda</rdfs:label>
    </owl:NamedIndividual>
    


    <!-- http://purl.obolibrary.org/obo/GAZ_00123873 -->

    <owl:NamedIndividual rdf:about="http://purl.obolibrary.org/obo/GAZ_00123873">
        <obo:RO_0001025 rdf:resource="http://purl.obolibrary.org/obo/GAZ_00031119"/>
        <obo:IAO_0000115>One of the 180 woredas in the Oromia Region of Ethiopia. Part of the Misraq (East) Shewa Zone located in the Great Rift Valley, Arsi Negele is bordered on the south by Shashamene, on the southwest by Lake Shala which separates it from Seraro, on the west from the Southern Nations, Nationalities and Peoples Region, on the north by Adami Tullu and Jido Kombolcha with which it shares the shores of Lakes Abijatta and Langano, and on the east by the Arsi Zone.</obo:IAO_0000115>
        <oboInOwl:hasOBONamespace>GAZ</oboInOwl:hasOBONamespace>
        <oboInOwl:id>GAZ:00123873</oboInOwl:id>
        <rdfs:label>Arsi Negele Woreda</rdfs:label>
    </owl:NamedIndividual>
    


    <!-- http://purl.obolibrary.org/obo/GAZ_00123874 -->

    <owl:NamedIndividual rdf:about="http://purl.obolibrary.org/obo/GAZ_00123874">
        <obo:RO_0001025 rdf:resource="http://purl.obolibrary.org/obo/GAZ_00031119"/>
        <obo:IAO_0000115>One of the 180 woredas in the Oromia Region of Ethiopia. Part of the Misraq Shewa Zone located in the Great Rift Valley, Fentale is bordered on the south by the Arsi Zone, on the southwest by Boset, on the northwest by the Amhara Region, and on the east by the Afar Region. The administrative center of Fentale is Metehara.</obo:IAO_0000115>
        <oboInOwl:hasOBONamespace>GAZ</oboInOwl:hasOBONamespace>
        <oboInOwl:id>GAZ:00123874</oboInOwl:id>
        <rdfs:label>Fentale Woreda</rdfs:label>
    </owl:NamedIndividual>
    


    <!-- http://purl.obolibrary.org/obo/GAZ_00123875 -->

    <owl:NamedIndividual rdf:about="http://purl.obolibrary.org/obo/GAZ_00123875">
        <obo:RO_0001025 rdf:resource="http://purl.obolibrary.org/obo/GAZ_00031123"/>
        <obo:IAO_0000115>One of the 180 woredas in the Oromia Region of Ethiopia. Part of the Misraq Welega Zone, Abe Dongoro is bordered on the south by Bila Seyo, on the west by Gida Kiremu, on the north by Amuru Jarte, and on the east by Jimma Horo. The woreda capital is Tulu Wayu.</obo:IAO_0000115>
        <oboInOwl:hasOBONamespace>GAZ</oboInOwl:hasOBONamespace>
        <oboInOwl:id>GAZ:00123875</oboInOwl:id>
        <rdfs:label>Abe Dongoro Woreda</rdfs:label>
    </owl:NamedIndividual>
    


    <!-- http://purl.obolibrary.org/obo/GAZ_00123876 -->

    <owl:NamedIndividual rdf:about="http://purl.obolibrary.org/obo/GAZ_00123876">
        <obo:RO_0001025 rdf:resource="http://purl.obolibrary.org/obo/GAZ_00031123"/>
        <obo:IAO_0000115>One of the 180 woredas in the Oromia Region of Ethiopia. Part of the Misraq (East) Welega Zone, Limmu is bordered on the south by an exclave of the Benishangul-Gumuz Region, on the southwest by Sasiga, on the west by the Benishangul-Gumuz Region, on the north by Ibantu, and on the east by Gida Kiremu. The administrative center of the woreda is Gelila.</obo:IAO_0000115>
        <oboInOwl:hasOBONamespace>GAZ</oboInOwl:hasOBONamespace>
        <oboInOwl:id>GAZ:00123876</oboInOwl:id>
        <rdfs:label>Limmu Woreda</rdfs:label>
    </owl:NamedIndividual>
    


    <!-- http://purl.obolibrary.org/obo/GAZ_00123877 -->

    <owl:NamedIndividual rdf:about="http://purl.obolibrary.org/obo/GAZ_00123877">
        <obo:RO_0001025 rdf:resource="http://purl.obolibrary.org/obo/GAZ_00031123"/>
        <obo:IAO_0000115>One of the 180 woredas in the Oromia Region of Ethiopia. Part of the Misraq Welega Zone, Nunu Kumba is bordered on the southwest by the Didessa River which separates it from the Illubabor Zone, on the northwest by Jimma Arjo, on the north by Guto Wayu, on the northeast by Wama Bonaya, and on the southeast by the Jimma Zone. The woreda capital is Nunu.</obo:IAO_0000115>
        <oboInOwl:hasOBONamespace>GAZ</oboInOwl:hasOBONamespace>
        <oboInOwl:id>GAZ:00123877</oboInOwl:id>
        <rdfs:label>Nunu Kumba Woreda</rdfs:label>
    </owl:NamedIndividual>
    


    <!-- http://purl.obolibrary.org/obo/GAZ_00123878 -->

    <owl:NamedIndividual rdf:about="http://purl.obolibrary.org/obo/GAZ_00123878">
        <obo:RO_0001025 rdf:resource="http://purl.obolibrary.org/obo/GAZ_00031123"/>
        <obo:IAO_0000115>One of the 180 woredas in the Oromia Region of Ethiopia. Part of the Misraq Welega Zone, Ibantu is bordered on the south by Limmu, on the west and north by the Benishangul-Gumuz Region, and on the east by Gida Kiremu. The administrative center of this woreda is Hinde.</obo:IAO_0000115>
        <oboInOwl:hasOBONamespace>GAZ</oboInOwl:hasOBONamespace>
        <oboInOwl:id>GAZ:00123878</oboInOwl:id>
        <rdfs:label>Ibantu Woreda</rdfs:label>
    </owl:NamedIndividual>
    


    <!-- http://purl.obolibrary.org/obo/GAZ_00123879 -->

    <owl:NamedIndividual rdf:about="http://purl.obolibrary.org/obo/GAZ_00123879">
        <obo:RO_0001025 rdf:resource="http://purl.obolibrary.org/obo/GAZ_00031123"/>
        <obo:IAO_0000115>One of the 180 woredas in the Oromia Region of Ethiopia. Part of the Misraq Welega Zone, Sasiga is bordered on the south by Diga Leka, on the west by the Benishangul-Gumuz Region, on the northwest by Limmu, on the north by an exclave of the Benishangul-Gumuz Region, and on the east by Guto Wayu.</obo:IAO_0000115>
        <oboInOwl:hasOBONamespace>GAZ</oboInOwl:hasOBONamespace>
        <oboInOwl:id>GAZ:00123879</oboInOwl:id>
        <rdfs:label>Sasiga Woreda</rdfs:label>
    </owl:NamedIndividual>
    


    <!-- http://purl.obolibrary.org/obo/GAZ_00123880 -->

    <owl:NamedIndividual rdf:about="http://purl.obolibrary.org/obo/GAZ_00123880">
        <obo:RO_0001025 rdf:resource="http://purl.obolibrary.org/obo/GAZ_00031123"/>
        <obo:IAO_0000115>One of the 180 woredas in the Oromia Region of Ethiopia. Part of the Misraq Welega Zone, Jimma Horo is bordered on the south by the Misraq Shewa Zone, on the southwest by Bila Seyo, on the west by Abe Dongoro, on the northwest by Amuru Jarte, on the northeast by Abay Chomen, on the east by Guduru, and on the southeast by Jimma Rare. The administrative center of the woreda is Shambu; other towns include Harato and Sekela.</obo:IAO_0000115>
        <oboInOwl:hasOBONamespace>GAZ</oboInOwl:hasOBONamespace>
        <oboInOwl:id>GAZ:00123880</oboInOwl:id>
        <rdfs:label>Jimma Horo Woreda</rdfs:label>
    </owl:NamedIndividual>
    


    <!-- http://purl.obolibrary.org/obo/GAZ_00123881 -->

    <owl:NamedIndividual rdf:about="http://purl.obolibrary.org/obo/GAZ_00123881">
        <obo:RO_0001025 rdf:resource="http://purl.obolibrary.org/obo/GAZ_00031123"/>
        <obo:IAO_0000115>One of the 180 woredas in the Oromia Region of Ethiopia. Part of the Misraq Welega Zone, Jimma Rare is bordered on the west by Jimma Horo, on the north by Guduru, on the east and south by the Guder River which separates it from the Mirab Shewa Zone.</obo:IAO_0000115>
        <oboInOwl:hasOBONamespace>GAZ</oboInOwl:hasOBONamespace>
        <oboInOwl:id>GAZ:00123881</oboInOwl:id>
        <rdfs:label>Jimma Rare Woreda</rdfs:label>
    </owl:NamedIndividual>
    


    <!-- http://purl.obolibrary.org/obo/GAZ_00123882 -->

    <owl:NamedIndividual rdf:about="http://purl.obolibrary.org/obo/GAZ_00123882">
        <obo:RO_0001025 rdf:resource="http://purl.obolibrary.org/obo/GAZ_00031123"/>
        <obo:IAO_0000115>One of the 180 woredas in the Oromia Region of Ethiopia. Part of the Misraq Welega Zone, Guduru is bordered on the south by Jimma Rare, on the southwest by Jimma Horo, on the west by Lake Finicha&apos;a, on the northwest by Abay Chomen, on the north by the Abay River which separates it from the Amhara Region, and on the east by the Guder River which separates it from the Mirab Shewa Zone. The administrative center is Guduru; other towns in Guduru include Dedu.</obo:IAO_0000115>
        <oboInOwl:hasOBONamespace>GAZ</oboInOwl:hasOBONamespace>
        <oboInOwl:id>GAZ:00123882</oboInOwl:id>
        <rdfs:label>Guduru Woreda</rdfs:label>
    </owl:NamedIndividual>
    


    <!-- http://purl.obolibrary.org/obo/GAZ_00123883 -->

    <owl:NamedIndividual rdf:about="http://purl.obolibrary.org/obo/GAZ_00123883">
        <obo:RO_0001025 rdf:resource="http://purl.obolibrary.org/obo/GAZ_00031123"/>
        <obo:IAO_0000115>One of the 180 woredas in the Oromia Region of Ethiopia. Part of the Misraq Welega Zone, Gida Kiremu is bordered on the south by Guto Wayu, on the west by Limmu, on the northwest by Ibantu, on the north by the Benishangul-Gumuz Region, on the east by Amuru Jarte, and on the southeast by Abe Dongoro. The administrative center of the woreda is Gida Ayana; other towns in Gida Kiremu include Gutin and Kiremu.</obo:IAO_0000115>
        <oboInOwl:hasOBONamespace>GAZ</oboInOwl:hasOBONamespace>
        <oboInOwl:id>GAZ:00123883</oboInOwl:id>
        <rdfs:label>Gida Kiremu Woreda</rdfs:label>
    </owl:NamedIndividual>
    


    <!-- http://purl.obolibrary.org/obo/GAZ_00123884 -->

    <owl:NamedIndividual rdf:about="http://purl.obolibrary.org/obo/GAZ_00123884">
        <obo:RO_0001025 rdf:resource="http://purl.obolibrary.org/obo/GAZ_00031123"/>
        <obo:IAO_0000115>One of the 180 woredas in the Oromia Region of Ethiopia. Part of the Misraq Welega Zone, Sibu Sire is bordered on the south by Wama Bonaya, on the west by Guto Wayu, and on the north and east by Bila Seyo. The woreda capital is Sire.</obo:IAO_0000115>
        <oboInOwl:hasOBONamespace>GAZ</oboInOwl:hasOBONamespace>
        <oboInOwl:id>GAZ:00123884</oboInOwl:id>
        <rdfs:label>Sibu Sire Woreda</rdfs:label>
    </owl:NamedIndividual>
    


    <!-- http://purl.obolibrary.org/obo/GAZ_00123885 -->

    <owl:NamedIndividual rdf:about="http://purl.obolibrary.org/obo/GAZ_00123885">
        <obo:RO_0001025 rdf:resource="http://purl.obolibrary.org/obo/GAZ_00031123"/>
        <obo:IAO_0000115>One of the 180 woredas in the Oromia Region of Ethiopia. Part of the Misraq Welega Zone, Wama Bonaya is bordered on the southwest by Nunu Kumba, on the west by Guto Wayu, on the northwest by Sibu Sire, on the north by Bila Seyo, on the northeast by the Mirab Shewa Zone, and on the southeast by the Jimma Zone. The woreda capital is Bilo; other towns in Wama Bonaya include Mote.</obo:IAO_0000115>
        <oboInOwl:hasOBONamespace>GAZ</oboInOwl:hasOBONamespace>
        <oboInOwl:id>GAZ:00123885</oboInOwl:id>
        <rdfs:label>Wama Bonaya Woreda</rdfs:label>
    </owl:NamedIndividual>
    


    <!-- http://purl.obolibrary.org/obo/GAZ_00123886 -->

    <owl:NamedIndividual rdf:about="http://purl.obolibrary.org/obo/GAZ_00123886">
        <obo:RO_0001025 rdf:resource="http://purl.obolibrary.org/obo/GAZ_00031123"/>
        <obo:IAO_0000115>One of the 180 woredas in the Oromia Region of Ethiopia. Part of the Misraq Welega Zone, Jimma Arjo is bordered on the southwest by the Didessa River which separates it from the Illubabor Zone, on the northwest by Diga Leka, on the northeast by Guto Wayu, and on the southeast by Nunu Kumba.</obo:IAO_0000115>
        <oboInOwl:hasOBONamespace>GAZ</oboInOwl:hasOBONamespace>
        <oboInOwl:id>GAZ:00123886</oboInOwl:id>
        <rdfs:label>Jimma Arjo Woreda</rdfs:label>
    </owl:NamedIndividual>
    


    <!-- http://purl.obolibrary.org/obo/GAZ_00123887 -->

    <owl:NamedIndividual rdf:about="http://purl.obolibrary.org/obo/GAZ_00123887">
        <obo:RO_0001025 rdf:resource="http://purl.obolibrary.org/obo/GAZ_00031123"/>
        <obo:IAO_0000115>One of the 180 woredas in the Oromia Region of Ethiopia. Part of the Misraq (East) Welega Zone, Bila Seyo is bordered on the south by Wama Bonaya, on the southwest by Sibu Sire, on the west by Guto Wayu, on the north by Abe Dongoro, on the northeast by Jimma Horo, and on the east by the Mirab Shewa Zone. The woreda capital is Ano; other towns in Bila Seyo include Bila and Jare.</obo:IAO_0000115>
        <oboInOwl:hasOBONamespace>GAZ</oboInOwl:hasOBONamespace>
        <oboInOwl:id>GAZ:00123887</oboInOwl:id>
        <rdfs:label>Bila Seyo Woreda</rdfs:label>
    </owl:NamedIndividual>
    


    <!-- http://purl.obolibrary.org/obo/GAZ_00123888 -->

    <owl:NamedIndividual rdf:about="http://purl.obolibrary.org/obo/GAZ_00123888">
        <obo:RO_0001025 rdf:resource="http://purl.obolibrary.org/obo/GAZ_00031123"/>
        <obo:IAO_0000115>One of the 180 woredas in the Oromia Region of Ethiopia. Part of the Misraq Welega Zone, Diga Leka is bordered on the south by an exclave of the Benishangul-Gumuz Region, on the west by the Didessa River which separates it from the Illubabor Zone on the southwest and the Mirab Welega Zone on the west, on the north by Sasiga, on the northeast by Guto Wayu and on the southeast by Jimma Arjo. The administrative center of the woreda is Gatama; other towns in Diga Leka include Arjo Gudetu and Diga.</obo:IAO_0000115>
        <oboInOwl:hasOBONamespace>GAZ</oboInOwl:hasOBONamespace>
        <oboInOwl:id>GAZ:00123888</oboInOwl:id>
        <rdfs:label>Diga Leka Woreda</rdfs:label>
    </owl:NamedIndividual>
    


    <!-- http://purl.obolibrary.org/obo/GAZ_00123889 -->

    <owl:NamedIndividual rdf:about="http://purl.obolibrary.org/obo/GAZ_00123889">
        <obo:RO_0001025 rdf:resource="http://purl.obolibrary.org/obo/GAZ_00031123"/>
        <obo:IAO_0000115>One of the 180 woredas in the Oromia Region of Ethiopia. Part of the Misraq Welega Zone, Guto Wayu is bordered on the south by Nunu Kumba, on the southwest by Jimma Arjo and Diga Leka, on the west by Sasiga, on the northwest by Limmu and Gida Kiremu, on the northeast by Bila Seyo, on the east by Sibu Sire, and on the southeast by Wama Bonaya. The woreda capital is Nekemte, which is also the Zonal capital; other towns include Gute.</obo:IAO_0000115>
        <oboInOwl:hasOBONamespace>GAZ</oboInOwl:hasOBONamespace>
        <oboInOwl:id>GAZ:00123889</oboInOwl:id>
        <rdfs:label>Guto Wayu Woreda</rdfs:label>
    </owl:NamedIndividual>
    


    <!-- http://purl.obolibrary.org/obo/GAZ_00123890 -->

    <owl:NamedIndividual rdf:about="http://purl.obolibrary.org/obo/GAZ_00123890">
        <obo:RO_0001025 rdf:resource="http://purl.obolibrary.org/obo/GAZ_00031123"/>
        <obo:IAO_0000115>One of the 180 woredas in the Oromia Region of Ethiopia. Part of the Misraq Welega Zone, Amuru Jarte is bordered on the south by Jimma Horo, on the southwest by Abe Dongoro, on the west by Gida Kiremu, on the north by the Abay River which separates it from the Amhara Region, and on the east by Abay Chomen. The woreda capital is Alibo; other towns in Amuru Jarte include Obora.</obo:IAO_0000115>
        <oboInOwl:hasOBONamespace>GAZ</oboInOwl:hasOBONamespace>
        <oboInOwl:id>GAZ:00123890</oboInOwl:id>
        <rdfs:label>Amuru Jarte Woreda</rdfs:label>
    </owl:NamedIndividual>
    


    <!-- http://purl.obolibrary.org/obo/GAZ_00123891 -->

    <owl:NamedIndividual rdf:about="http://purl.obolibrary.org/obo/GAZ_00123891">
        <obo:RO_0001025 rdf:resource="http://purl.obolibrary.org/obo/GAZ_00031123"/>
        <obo:IAO_0000115>One of the 180 woredas in the Oromia Region of Ethiopia. Part of the Misraq Welega Zone, Abay Chomen is bordered on the south by Lake Finicha&apos;a (created when Finicha&apos;a Dam flooded the Chomen swamp), on the southwest by Jimma Horo, on the northwest by Amuru Jarte, on the north by the Abay River which separates it from the Amhara Region, and on the east and south by Guduru. The woreda capital is Finicha&apos;a; other towns in Abay Chomen include Finicha&apos;a Camp.</obo:IAO_0000115>
        <oboInOwl:hasOBONamespace>GAZ</oboInOwl:hasOBONamespace>
        <oboInOwl:id>GAZ:00123891</oboInOwl:id>
        <rdfs:label>Abay Chomen Woreda</rdfs:label>
    </owl:NamedIndividual>
    


    <!-- http://purl.obolibrary.org/obo/GAZ_00123892 -->

    <owl:NamedIndividual rdf:about="http://purl.obolibrary.org/obo/GAZ_00123892">
        <obo:RO_0001025 rdf:resource="http://purl.obolibrary.org/obo/GAZ_00031122"/>
        <obo:IAO_0000115>One of the 180 woredas in the Oromia Region of Ethiopia. Part of the Semien Shewa Zone, Hidabu Abote is bordered on the south by Kuyu, on the west by Wara Jarso, on the north by the Jamma River which separates it from Dera, and on the east by Gegem. The major town in Hidabu Abote is Ejere.</obo:IAO_0000115>
        <oboInOwl:hasOBONamespace>GAZ</oboInOwl:hasOBONamespace>
        <oboInOwl:id>GAZ:00123892</oboInOwl:id>
        <rdfs:label>Hidabu Abote Woreda</rdfs:label>
    </owl:NamedIndividual>
    


    <!-- http://purl.obolibrary.org/obo/GAZ_00123893 -->

    <owl:NamedIndividual rdf:about="http://purl.obolibrary.org/obo/GAZ_00123893">
        <obo:RO_0001025 rdf:resource="http://purl.obolibrary.org/obo/GAZ_00031122"/>
        <obo:IAO_0000115>One of the 180 woredas in the Oromia Region of Ethiopia. Part of the Semien Shewa Zone, Wara Jarso is bordered on the south by Kuyu, on the west by the Muger River which separates it from the Misraq Welega Zone, on the north by the Abay River which separates it from the Amhara Region, on the northeast by the Jamma River which separates it from Dera, and on the east by Hidabu Abote. Towns in Wara Jarso include Filiklik, Goha Tsion and Tullu Milki.</obo:IAO_0000115>
        <oboInOwl:hasOBONamespace>GAZ</oboInOwl:hasOBONamespace>
        <oboInOwl:id>GAZ:00123893</oboInOwl:id>
        <rdfs:label>Wara Jarso Woreda</rdfs:label>
    </owl:NamedIndividual>
    


    <!-- http://purl.obolibrary.org/obo/GAZ_00123894 -->

    <owl:NamedIndividual rdf:about="http://purl.obolibrary.org/obo/GAZ_00123894">
        <obo:RO_0001025 rdf:resource="http://purl.obolibrary.org/obo/GAZ_00031122"/>
        <obo:IAO_0000115>One of the 180 woredas in the Oromia Region of Ethiopia. Part of the Semien Shewa Zone, Wuchalena Jido is bordered on the south by Berehna Aleltu, on the west by Mulona Sululta, on the northwest by Yaya Gulelena Debre Liban, on the northeast by the Amhara Region, on the east by Abichuna Gne&apos;a, and on the southeast by Kembibit. Towns in Wuchalena Jido include Muka and Turi.</obo:IAO_0000115>
        <oboInOwl:hasOBONamespace>GAZ</oboInOwl:hasOBONamespace>
        <oboInOwl:id>GAZ:00123894</oboInOwl:id>
        <rdfs:label>Wuchalena Jido Woreda</rdfs:label>
    </owl:NamedIndividual>
    


    <!-- http://purl.obolibrary.org/obo/GAZ_00123895 -->

    <owl:NamedIndividual rdf:about="http://purl.obolibrary.org/obo/GAZ_00123895">
        <obo:RO_0001025 rdf:resource="http://purl.obolibrary.org/obo/GAZ_00031122"/>
        <obo:IAO_0000115>One of the 180 woredas in the Oromia Region of Ethiopia. Part of the Semien Shewa Zone, Yaya Gulele and Debre Liban is bordered on the south by Mulona Sululta, on the southwest by the Muger River which separates it from the Mirab Shewa Zone, on the west by Gegem, on the north by Gerar Jarso, on the east by the Amhara Region, and on the southeast by Wuchalena Jido. Towns in Yaya Gulele and Debre Liban include Debre Tsige and Fital.</obo:IAO_0000115>
        <oboInOwl:hasOBONamespace>GAZ</oboInOwl:hasOBONamespace>
        <oboInOwl:id>GAZ:00123895</oboInOwl:id>
        <rdfs:label>Yaya Gulelena Debre Liban Woreda</rdfs:label>
    </owl:NamedIndividual>
    


    <!-- http://purl.obolibrary.org/obo/GAZ_00123896 -->

    <owl:NamedIndividual rdf:about="http://purl.obolibrary.org/obo/GAZ_00123896">
        <obo:RO_0001025 rdf:resource="http://purl.obolibrary.org/obo/GAZ_00031122"/>
        <obo:IAO_0000115>One of the 180 woredas in the Oromia Region of Ethiopia. Part of the Semien Shewa Zone, Gerar Jarso is bordered on the south by Yaya Gulelena Debre Liban, on the west by Gegem, and on the east by the Amhara Region. The major town in Gerar Jarso is Fiche.</obo:IAO_0000115>
        <oboInOwl:hasOBONamespace>GAZ</oboInOwl:hasOBONamespace>
        <oboInOwl:id>GAZ:00123896</oboInOwl:id>
        <rdfs:label>Gerar Jarso Woreda</rdfs:label>
    </owl:NamedIndividual>
    


    <!-- http://purl.obolibrary.org/obo/GAZ_00123897 -->

    <owl:NamedIndividual rdf:about="http://purl.obolibrary.org/obo/GAZ_00123897">
        <obo:RO_0001025 rdf:resource="http://purl.obolibrary.org/obo/GAZ_00031122"/>
        <obo:IAO_0000115>One of the 180 woredas (districts) in the Oromia Region of Ethiopia. Part of the Semien Shewa Zone, Kuyu is bordered on the south and west by the Muger River which separates it from the Misraq Welega Zone, on the north by Wara Jarso, on the northeast by Hidabu Abote, and on the east by Gegem. The administrative center of Kuyu is Gebre Guracha.</obo:IAO_0000115>
        <oboInOwl:hasOBONamespace>GAZ</oboInOwl:hasOBONamespace>
        <oboInOwl:id>GAZ:00123897</oboInOwl:id>
        <rdfs:label>Kuyu Woreda</rdfs:label>
    </owl:NamedIndividual>
    


    <!-- http://purl.obolibrary.org/obo/GAZ_00123898 -->

    <owl:NamedIndividual rdf:about="http://purl.obolibrary.org/obo/GAZ_00123898">
        <obo:RO_0001025 rdf:resource="http://purl.obolibrary.org/obo/GAZ_00031122"/>
        <obo:IAO_0000115>One of the 180 woredas in the Oromia Region of Ethiopia. Part of the Semien Shewa Zone, Dera is bordered on the south by the Jamma River which separates it from Hidabu Abote and Wara Jarso, on the west, north and east by the Amhara Region; the Abay River defines the western boundary, and its tributary the Walaqa the northern. The major town in Dera is Gundo Meskel.</obo:IAO_0000115>
        <oboInOwl:hasOBONamespace>GAZ</oboInOwl:hasOBONamespace>
        <oboInOwl:id>GAZ:00123898</oboInOwl:id>
        <rdfs:label>Dera Woreda</rdfs:label>
    </owl:NamedIndividual>
    


    <!-- http://purl.obolibrary.org/obo/GAZ_00123899 -->

    <owl:NamedIndividual rdf:about="http://purl.obolibrary.org/obo/GAZ_00123899">
        <obo:RO_0001025 rdf:resource="http://purl.obolibrary.org/obo/GAZ_00031122"/>
        <obo:IAO_0000115>One of the 180 woredas in the Oromia Region of Ethiopia. Part of the Semien Shewa Zone, Kembibit is bordered on the south by Berhena Aleltu, on the west by Wuchalena Jido, on the north by Abichuna Gne&apos;a, and on the east by the Amhara Region. Towns in Kembibit include Hamus Gebeya, Kotu and Sheno.</obo:IAO_0000115>
        <oboInOwl:hasOBONamespace>GAZ</oboInOwl:hasOBONamespace>
        <oboInOwl:id>GAZ:00123899</oboInOwl:id>
        <rdfs:label>Kembibit Woreda</rdfs:label>
    </owl:NamedIndividual>
    


    <!-- http://purl.obolibrary.org/obo/GAZ_00123900 -->

    <owl:NamedIndividual rdf:about="http://purl.obolibrary.org/obo/GAZ_00123900">
        <obo:RO_0001025 rdf:resource="http://purl.obolibrary.org/obo/GAZ_00031122"/>
        <obo:IAO_0000115>One of the 180 woredas in the Oromia Region of Ethiopia. Part of the Semien Shewa Zone, Berehna Aleltu is bordered on the south by the Misraq Shewa Zone, on the southwest by the city of Addis Ababa, on the west by Mulona Sululta, on the north by Wuchalena Jido, on the northeast by Kembibit, and on the east by the Amhara Region.</obo:IAO_0000115>
        <oboInOwl:hasOBONamespace>GAZ</oboInOwl:hasOBONamespace>
        <oboInOwl:id>GAZ:00123900</oboInOwl:id>
        <rdfs:label>Berehna Aleltu Woreda</rdfs:label>
    </owl:NamedIndividual>
    


    <!-- http://purl.obolibrary.org/obo/GAZ_00123901 -->

    <owl:NamedIndividual rdf:about="http://purl.obolibrary.org/obo/GAZ_00123901">
        <obo:RO_0001025 rdf:resource="http://purl.obolibrary.org/obo/GAZ_00031122"/>
        <obo:IAO_0000115>One of the 180 woredas in the Oromia Region of Ethiopia. Part of the Semien Shewa Zone, Abichuna Gne&apos;a is bordered on the south by Kembibit, on the west by Wuchalena Jido, and on the north and east by the Amhara Region. The major town in Abichuna Gne&apos;a is Mendida.</obo:IAO_0000115>
        <oboInOwl:hasOBONamespace>GAZ</oboInOwl:hasOBONamespace>
        <oboInOwl:id>GAZ:00123901</oboInOwl:id>
        <rdfs:label>Abichuna Gne&apos;a Woreda</rdfs:label>
    </owl:NamedIndividual>
    


    <!-- http://purl.obolibrary.org/obo/GAZ_00123902 -->

    <owl:NamedIndividual rdf:about="http://purl.obolibrary.org/obo/GAZ_00123902">
        <obo:RO_0001025 rdf:resource="http://purl.obolibrary.org/obo/GAZ_00031122"/>
        <obo:IAO_0000115>One of the 180 woredas in the Oromia Region of Ethiopia. Part of the Semien Shewa Zone, Gegem is bordered on the south by the Muger River which separates it from the Misraq Welega Zone, on the west by Kuyu, on the northwest by Hidabu Abote, on the north by the Jimma River which separates it from the Amhara Region, on the northeast by Gerar Jarso, and on the east by Yaya Gulelena Debre Liban. Towns in Gegem include Alidoro and Anbiso.</obo:IAO_0000115>
        <oboInOwl:hasOBONamespace>GAZ</oboInOwl:hasOBONamespace>
        <oboInOwl:id>GAZ:00123902</oboInOwl:id>
        <rdfs:label>Gegem Woreda</rdfs:label>
    </owl:NamedIndividual>
    


    <!-- http://purl.obolibrary.org/obo/GAZ_00123903 -->

    <owl:NamedIndividual rdf:about="http://purl.obolibrary.org/obo/GAZ_00123903">
        <obo:RO_0001025 rdf:resource="http://purl.obolibrary.org/obo/GAZ_00031116"/>
        <obo:IAO_0000115>One of the 180 woredas in the Oromia Region of Ethiopia. Part of the Misraq (East) Hararghe Zone, Babille is bordered on the south and east by the Somali Region, on the west by Fedis, and on the north by Gursum; the Fafen River defines a portion of Babille&apos;s eastern border. The woreda capital is Babille.</obo:IAO_0000115>
        <oboInOwl:hasOBONamespace>GAZ</oboInOwl:hasOBONamespace>
        <oboInOwl:id>GAZ:00123903</oboInOwl:id>
        <rdfs:label>Babille Woreda</rdfs:label>
    </owl:NamedIndividual>
    


    <!-- http://purl.obolibrary.org/obo/GAZ_00123904 -->

    <owl:NamedIndividual rdf:about="http://purl.obolibrary.org/obo/GAZ_00123904">
        <obo:RO_0001025 rdf:resource="http://purl.obolibrary.org/obo/GAZ_00031116"/>
        <obo:IAO_0000115>One of the 180 woredas in the Oromia Region of Ethiopia. Part of the Misraq (East) Hararghe Zone, Deder is bordered on the south by Malka Balo, on the west by the Mirab (West) Hararghe Zone, on the north by Goro Gutu, on the east by Meta, and on the southeast by Bedeno. Towns include Kobo.</obo:IAO_0000115>
        <oboInOwl:hasOBONamespace>GAZ</oboInOwl:hasOBONamespace>
        <oboInOwl:id>GAZ:00123904</oboInOwl:id>
        <rdfs:label>Deder Woreda</rdfs:label>
    </owl:NamedIndividual>
    


    <!-- http://purl.obolibrary.org/obo/GAZ_00123905 -->

    <owl:NamedIndividual rdf:about="http://purl.obolibrary.org/obo/GAZ_00123905">
        <obo:RO_0001025 rdf:resource="http://purl.obolibrary.org/obo/GAZ_00031116"/>
        <obo:IAO_0000115>One of the 180 woredas in the Oromia Region of Ethiopia. Part of the Misraq (East) Hararghe Zone, Bedeno is bordered on the south by Gola Odana Meyumuluke, on the southwest by Malka Balo, on the west by Deder, on the northwest by Meta, on the north by Jarso, on the northeast by Kurfa Chele, and on the east by Girawa. Towns include Furda.</obo:IAO_0000115>
        <oboInOwl:hasOBONamespace>GAZ</oboInOwl:hasOBONamespace>
        <oboInOwl:id>GAZ:00123905</oboInOwl:id>
        <rdfs:label>Bedeno Woreda</rdfs:label>
    </owl:NamedIndividual>
    


    <!-- http://purl.obolibrary.org/obo/GAZ_00123906 -->

    <owl:NamedIndividual rdf:about="http://purl.obolibrary.org/obo/GAZ_00123906">
        <obo:RO_0001025 rdf:resource="http://purl.obolibrary.org/obo/GAZ_00031125"/>
        <obo:IAO_0000115>One of the 180 woredas in the Oromia Region of Ethiopia. Part of the Mirab Shewa Zone, Ginde Beret is bordered on the south by Ambo, on the west by the Guder River which separates it from the Misraq Welega Zone, on the north by the Abay River which separates it from the Amhara Region, on the east by the Muger River which separates it from the Semien Shewa Zone, and on the southeast by Jedlu. The major town in Ginde Beret is Kachise.</obo:IAO_0000115>
        <oboInOwl:hasOBONamespace>GAZ</oboInOwl:hasOBONamespace>
        <oboInOwl:id>GAZ:00123906</oboInOwl:id>
        <rdfs:label>Ginde Beret Woreda</rdfs:label>
    </owl:NamedIndividual>
    


    <!-- http://purl.obolibrary.org/obo/GAZ_00123907 -->

    <owl:NamedIndividual rdf:about="http://purl.obolibrary.org/obo/GAZ_00123907">
        <obo:RO_0001025 rdf:resource="http://purl.obolibrary.org/obo/GAZ_00123543"/>
        <obo:RO_0001025 rdf:resource="http://purl.obolibrary.org/obo/GAZ_00123746"/>
        <obo:RO_0001025 rdf:resource="http://purl.obolibrary.org/obo/GAZ_00123750"/>
        <obo:IAO_0000115>An isolated, extinct silicic volcanic mountain in southeastern Ethiopia. The highest point in the Arsi Zone of the Oromia Region, and located on the border between the Hitosa and Tiyo wored. Although this mountain is located south of the Great Rift Valley, along with Mount Gugu to the north and Mount Kaka to the south, it is considered, geologically speaking, part of the Ethiopian highlands.</obo:IAO_0000115>
        <oboInOwl:hasOBONamespace>GAZ</oboInOwl:hasOBONamespace>
        <oboInOwl:id>GAZ:00123907</oboInOwl:id>
        <rdfs:label>Mount Chilalo</rdfs:label>
    </owl:NamedIndividual>
    


    <!-- http://purl.obolibrary.org/obo/GAZ_00123908 -->

    <owl:NamedIndividual rdf:about="http://purl.obolibrary.org/obo/GAZ_00123908">
        <obo:RO_0001025 rdf:resource="http://purl.obolibrary.org/obo/GAZ_00123756"/>
        <obo:IAO_0000115>A karst cave. The longest cave in Ethiopia. It is situated in the Bale province in southeastern Ethiopia through which the Web River flows. It sinks at the Ayiew Maco entrance and reappears at the Holuca resurgence 1 km away.</obo:IAO_0000115>
        <oboInOwl:hasOBONamespace>GAZ</oboInOwl:hasOBONamespace>
        <oboInOwl:id>GAZ:00123908</oboInOwl:id>
        <rdfs:label>Sof Omar Caves</rdfs:label>
    </owl:NamedIndividual>
    


    <!-- http://purl.obolibrary.org/obo/GAZ_00123909 -->

    <owl:NamedIndividual rdf:about="http://purl.obolibrary.org/obo/GAZ_00123909">
        <obo:RO_0001025 rdf:resource="http://purl.obolibrary.org/obo/GAZ_00052524"/>
        <obo:IAO_0000115>A lake.</obo:IAO_0000115>
        <oboInOwl:hasOBONamespace>GAZ</oboInOwl:hasOBONamespace>
        <oboInOwl:id>GAZ:00123909</oboInOwl:id>
        <rdfs:label>Lake Alemaya</rdfs:label>
    </owl:NamedIndividual>
    


    <!-- http://purl.obolibrary.org/obo/GAZ_00123910 -->

    <owl:NamedIndividual rdf:about="http://purl.obolibrary.org/obo/GAZ_00123910">
        <obo:RO_0001025 rdf:resource="http://purl.obolibrary.org/obo/GAZ_00123871"/>
        <obo:IAO_0000115>A lake.</obo:IAO_0000115>
        <oboInOwl:hasOBONamespace>GAZ</oboInOwl:hasOBONamespace>
        <oboInOwl:id>GAZ:00123910</oboInOwl:id>
        <rdfs:label>Lake Chelaka</rdfs:label>
    </owl:NamedIndividual>
    


    <!-- http://purl.obolibrary.org/obo/GAZ_00123911 -->

    <owl:NamedIndividual rdf:about="http://purl.obolibrary.org/obo/GAZ_00123911">
        <obo:RO_0001025 rdf:resource="http://purl.obolibrary.org/obo/GAZ_00123891"/>
        <obo:IAO_0000115>An artificial lake created when Finicha&apos;a Dam flooded the Chomen swamp.</obo:IAO_0000115>
        <oboInOwl:hasOBONamespace>GAZ</oboInOwl:hasOBONamespace>
        <oboInOwl:id>GAZ:00123911</oboInOwl:id>
        <rdfs:label>Lake Finicha&apos;a</rdfs:label>
    </owl:NamedIndividual>
    


    <!-- http://purl.obolibrary.org/obo/GAZ_00123912 -->

    <owl:NamedIndividual rdf:about="http://purl.obolibrary.org/obo/GAZ_00123912">
        <obo:RO_0001025 rdf:resource="http://purl.obolibrary.org/obo/GAZ_00123796"/>
        <obo:IAO_0000115>A lake.</obo:IAO_0000115>
        <oboInOwl:hasOBONamespace>GAZ</oboInOwl:hasOBONamespace>
        <oboInOwl:id>GAZ:00123912</oboInOwl:id>
        <rdfs:label>Lake Cheleleki</rdfs:label>
    </owl:NamedIndividual>
    


    <!-- http://purl.obolibrary.org/obo/GAZ_00123913 -->

    <owl:NamedIndividual rdf:about="http://purl.obolibrary.org/obo/GAZ_00123913">
        <obo:RO_0001025 rdf:resource="http://purl.obolibrary.org/obo/GAZ_00123824"/>
        <obo:IAO_0000115>A protected area.</obo:IAO_0000115>
        <oboInOwl:hasOBONamespace>GAZ</oboInOwl:hasOBONamespace>
        <oboInOwl:id>GAZ:00123913</oboInOwl:id>
        <rdfs:label>Menagesha National Forest</rdfs:label>
    </owl:NamedIndividual>
    


    <!-- http://purl.obolibrary.org/obo/GAZ_00124218 -->

    <owl:NamedIndividual rdf:about="http://purl.obolibrary.org/obo/GAZ_00124218">
        <obo:RO_0001025 rdf:resource="http://purl.obolibrary.org/obo/GAZ_00000007"/>
        <obo:IAO_0000115>A series of hills in Baringo District, Kenya.</obo:IAO_0000115>
        <oboInOwl:hasOBONamespace>GAZ</oboInOwl:hasOBONamespace>
        <oboInOwl:id>GAZ:00124218</oboInOwl:id>
        <rdfs:label>Tugen Hills</rdfs:label>
    </owl:NamedIndividual>
    


    <!-- http://purl.obolibrary.org/obo/GAZ_00124306 -->

    <owl:NamedIndividual rdf:about="http://purl.obolibrary.org/obo/GAZ_00124306">
        <obo:RO_0001025 rdf:resource="http://purl.obolibrary.org/obo/GAZ_00000007"/>
        <obo:IAO_0000115>A steep natural cliff approximately 3,000 m high, running along the western edge of the Great Rift Valley in Kenya.</obo:IAO_0000115>
        <oboInOwl:hasOBONamespace>GAZ</oboInOwl:hasOBONamespace>
        <oboInOwl:id>GAZ:00124306</oboInOwl:id>
        <rdfs:label>Mau Escarpment</rdfs:label>
    </owl:NamedIndividual>
    


    <!-- http://purl.obolibrary.org/obo/GAZ_00124307 -->

    <owl:NamedIndividual rdf:about="http://purl.obolibrary.org/obo/GAZ_00124307">
        <obo:RO_0001025 rdf:resource="http://purl.obolibrary.org/obo/GAZ_00124306"/>
        <obo:IAO_0000115>A forest complex in the Rift Valley of Kenya. It is the largest indigenous montane forest in East Africa. The Mau Forest complex has an area of 273300 ha.</obo:IAO_0000115>
        <oboInOwl:hasOBONamespace>GAZ</oboInOwl:hasOBONamespace>
        <oboInOwl:id>GAZ:00124307</oboInOwl:id>
        <rdfs:label>Mau Forest</rdfs:label>
    </owl:NamedIndividual>
    


    <!-- http://purl.obolibrary.org/obo/GAZ_00124567 -->

    <owl:NamedIndividual rdf:about="http://purl.obolibrary.org/obo/GAZ_00124567">
        <obo:RO_0001025 rdf:resource="http://purl.obolibrary.org/obo/GAZ_00015452"/>
        <oboInOwl:hasOBONamespace>GAZ</oboInOwl:hasOBONamespace>
        <oboInOwl:id>GAZ:00124567</oboInOwl:id>
        <rdfs:label>Napoleon Gulf</rdfs:label>
    </owl:NamedIndividual>
    


    <!-- http://purl.obolibrary.org/obo/GAZ_00124568 -->

    <owl:NamedIndividual rdf:about="http://purl.obolibrary.org/obo/GAZ_00124568">
        <obo:RO_0001025 rdf:resource="http://purl.obolibrary.org/obo/GAZ_00015453"/>
        <obo:IAO_0000115>The largest of the Buvuma Islands.</obo:IAO_0000115>
        <oboInOwl:hasOBONamespace>GAZ</oboInOwl:hasOBONamespace>
        <oboInOwl:id>GAZ:00124568</oboInOwl:id>
        <rdfs:label>Buvuma Island</rdfs:label>
    </owl:NamedIndividual>
    


    <!-- http://purl.obolibrary.org/obo/GAZ_00124569 -->

    <owl:NamedIndividual rdf:about="http://purl.obolibrary.org/obo/GAZ_00124569">
        <obo:RO_0001025 rdf:resource="http://purl.obolibrary.org/obo/GAZ_00015452"/>
        <obo:RO_0001025 rdf:resource="http://purl.obolibrary.org/obo/GAZ_00015453"/>
        <obo:IAO_0000115>One of the Buvuma Islands.</obo:IAO_0000115>
        <oboInOwl:hasOBONamespace>GAZ</oboInOwl:hasOBONamespace>
        <oboInOwl:id>GAZ:00124569</oboInOwl:id>
        <rdfs:label>Bugaia Island</rdfs:label>
    </owl:NamedIndividual>
    


    <!-- http://purl.obolibrary.org/obo/GAZ_00124570 -->

    <owl:NamedIndividual rdf:about="http://purl.obolibrary.org/obo/GAZ_00124570">
        <obo:RO_0001025 rdf:resource="http://purl.obolibrary.org/obo/GAZ_00015452"/>
        <obo:RO_0001025 rdf:resource="http://purl.obolibrary.org/obo/GAZ_00015453"/>
        <obo:IAO_0000115>One of the Buvuma Islands.</obo:IAO_0000115>
        <oboInOwl:hasOBONamespace>GAZ</oboInOwl:hasOBONamespace>
        <oboInOwl:id>GAZ:00124570</oboInOwl:id>
        <rdfs:label>Lingira Island</rdfs:label>
    </owl:NamedIndividual>
    


    <!-- http://purl.obolibrary.org/obo/GAZ_00124571 -->

    <owl:NamedIndividual rdf:about="http://purl.obolibrary.org/obo/GAZ_00124571">
        <obo:RO_0001025 rdf:resource="http://purl.obolibrary.org/obo/GAZ_00015452"/>
        <obo:RO_0001025 rdf:resource="http://purl.obolibrary.org/obo/GAZ_00015453"/>
        <obo:IAO_0000115>One of the Buvuma Islands.</obo:IAO_0000115>
        <oboInOwl:hasOBONamespace>GAZ</oboInOwl:hasOBONamespace>
        <oboInOwl:id>GAZ:00124571</oboInOwl:id>
        <rdfs:label>Namiti Island</rdfs:label>
    </owl:NamedIndividual>
    


    <!-- http://purl.obolibrary.org/obo/GAZ_00136138 -->

    <owl:NamedIndividual rdf:about="http://purl.obolibrary.org/obo/GAZ_00136138">
        <obo:RO_0001025 rdf:resource="http://purl.obolibrary.org/obo/GAZ_00000007"/>
        <obo:IAO_0000115>A region along the East African Rift in Tanzania, located in a spreading zone at the intersection of branches of the African and Somali tectonic plates.</obo:IAO_0000115>
        <oboInOwl:hasOBONamespace>GAZ</oboInOwl:hasOBONamespace>
        <oboInOwl:id>GAZ:00136138</oboInOwl:id>
        <rdfs:label>Crater Highlands</rdfs:label>
    </owl:NamedIndividual>
    


    <!-- http://purl.obolibrary.org/obo/GAZ_00136139 -->

    <owl:NamedIndividual rdf:about="http://purl.obolibrary.org/obo/GAZ_00136139">
        <obo:RO_0001025 rdf:resource="http://purl.obolibrary.org/obo/GAZ_00136138"/>
        <oboInOwl:hasOBONamespace>GAZ</oboInOwl:hasOBONamespace>
        <oboInOwl:id>GAZ:00136139</oboInOwl:id>
        <rdfs:label>Ela Naibori Crater</rdfs:label>
    </owl:NamedIndividual>
    


    <!-- http://purl.obolibrary.org/obo/GAZ_00136140 -->

    <owl:NamedIndividual rdf:about="http://purl.obolibrary.org/obo/GAZ_00136140">
        <obo:RO_0001025 rdf:resource="http://purl.obolibrary.org/obo/GAZ_00136138"/>
        <obo:IAO_0000115>A volcano located in Tanzania in the Crater Highlands region. It is at the southeastern edge of Lake Natron in Africa&apos;s Great Rift Valley.</obo:IAO_0000115>
        <oboInOwl:hasOBONamespace>GAZ</oboInOwl:hasOBONamespace>
        <oboInOwl:id>GAZ:00136140</oboInOwl:id>
        <rdfs:label>Gelai Volcano</rdfs:label>
    </owl:NamedIndividual>
    


    <!-- http://purl.obolibrary.org/obo/GAZ_00136141 -->

    <owl:NamedIndividual rdf:about="http://purl.obolibrary.org/obo/GAZ_00136141">
        <obo:RO_0001025 rdf:resource="http://purl.obolibrary.org/obo/GAZ_00136138"/>
        <oboInOwl:hasOBONamespace>GAZ</oboInOwl:hasOBONamespace>
        <oboInOwl:id>GAZ:00136141</oboInOwl:id>
        <rdfs:label>Meto Hills</rdfs:label>
    </owl:NamedIndividual>
    


    <!-- http://purl.obolibrary.org/obo/GAZ_00176005 -->

    <owl:NamedIndividual rdf:about="http://purl.obolibrary.org/obo/GAZ_00176005">
        <obo:RO_0001025 rdf:resource="http://purl.obolibrary.org/obo/GAZ_00007862"/>
        <obo:IAO_0000115>An island in the northern Gulf of Aqaba off the shore of Egypt&apos;s eastern Sinai Peninsula.</obo:IAO_0000115>
        <oboInOwl:hasOBONamespace>GAZ</oboInOwl:hasOBONamespace>
        <oboInOwl:id>GAZ:00176005</oboInOwl:id>
        <rdfs:label>Pharaoh&apos;s Island</rdfs:label>
    </owl:NamedIndividual>
    


    <!-- http://purl.obolibrary.org/obo/GAZ_00193785 -->

    <owl:NamedIndividual rdf:about="http://purl.obolibrary.org/obo/GAZ_00193785">
        <obo:RO_0001025 rdf:resource="http://purl.obolibrary.org/obo/GAZ_00007520"/>
        <obo:IAO_0000115>A river. A tributary of the Jordan River.</obo:IAO_0000115>
        <oboInOwl:hasOBONamespace>GAZ</oboInOwl:hasOBONamespace>
        <oboInOwl:id>GAZ:00193785</oboInOwl:id>
        <rdfs:label>Banias River</rdfs:label>
    </owl:NamedIndividual>
    


    <!-- http://purl.obolibrary.org/obo/GAZ_00193791 -->

    <owl:NamedIndividual rdf:about="http://purl.obolibrary.org/obo/GAZ_00193791">
        <obo:IAO_0000115>The lowest nature reserve in the world, with a spectacular array of scenery near the east cost of the Dead Sea. The reserve is located within the deep Wadi Mujib gorge, which enters the Dead Sea at 410 m below sea level. The Reserve extends to the Kerak and Madaba mountains to the north and south.</obo:IAO_0000115>
        <oboInOwl:hasOBONamespace>GAZ</oboInOwl:hasOBONamespace>
        <oboInOwl:id>GAZ:00193791</oboInOwl:id>
        <rdfs:label>Mujib Nature Reserve</rdfs:label>
    </owl:NamedIndividual>
    


    <!-- http://purl.obolibrary.org/obo/GAZ_00193804 -->

    <owl:NamedIndividual rdf:about="http://purl.obolibrary.org/obo/GAZ_00193804">
        <obo:RO_0001025 rdf:resource="http://purl.obolibrary.org/obo/GAZ_00007862"/>
        <obo:IAO_0000115>A protected area located on the Red Sea south of Eilat.</obo:IAO_0000115>
        <oboInOwl:hasOBONamespace>GAZ</oboInOwl:hasOBONamespace>
        <oboInOwl:id>GAZ:00193804</oboInOwl:id>
        <rdfs:label>Coral Beach Nature Reserve</rdfs:label>
    </owl:NamedIndividual>
    


    <!-- http://purl.obolibrary.org/obo/GAZ_00193854 -->

    <owl:NamedIndividual rdf:about="http://purl.obolibrary.org/obo/GAZ_00193854">
        <obo:RO_0001025 rdf:resource="http://purl.obolibrary.org/obo/GAZ_00010533"/>
        <obo:IAO_0000115>A protected area. An archeological site. A World Heritage Site.</obo:IAO_0000115>
        <oboInOwl:hasOBONamespace>GAZ</oboInOwl:hasOBONamespace>
        <oboInOwl:id>GAZ:00193854</oboInOwl:id>
        <rdfs:label>Megiddo National Park</rdfs:label>
    </owl:NamedIndividual>
    


    <!-- http://purl.obolibrary.org/obo/GAZ_00193855 -->

    <owl:NamedIndividual rdf:about="http://purl.obolibrary.org/obo/GAZ_00193855">
        <obo:RO_0001025 rdf:resource="http://purl.obolibrary.org/obo/GAZ_00010533"/>
        <obo:IAO_0000115>A protected area. An archeological site.</obo:IAO_0000115>
        <oboInOwl:hasOBONamespace>GAZ</oboInOwl:hasOBONamespace>
        <oboInOwl:id>GAZ:00193855</oboInOwl:id>
        <rdfs:label>Ma&apos;ayan Harod National Park</rdfs:label>
    </owl:NamedIndividual>
    


    <!-- http://purl.obolibrary.org/obo/GAZ_00193856 -->

    <owl:NamedIndividual rdf:about="http://purl.obolibrary.org/obo/GAZ_00193856">
        <obo:RO_0001025 rdf:resource="http://purl.obolibrary.org/obo/GAZ_00193855"/>
        <obo:IAO_0000115>A spring. It emerges from a rocky cave on the slope of Mount Gilboa.</obo:IAO_0000115>
        <oboInOwl:hasOBONamespace>GAZ</oboInOwl:hasOBONamespace>
        <oboInOwl:id>GAZ:00193856</oboInOwl:id>
        <rdfs:label>Ma&apos;ayan Harod</rdfs:label>
    </owl:NamedIndividual>
    


    <!-- http://purl.obolibrary.org/obo/GAZ_00193866 -->

    <owl:NamedIndividual rdf:about="http://purl.obolibrary.org/obo/GAZ_00193866">
        <obo:RO_0001025 rdf:resource="http://purl.obolibrary.org/obo/GAZ_00044915"/>
        <obo:IAO_0000115>A protected area. An archeological site.</obo:IAO_0000115>
        <oboInOwl:hasOBONamespace>GAZ</oboInOwl:hasOBONamespace>
        <oboInOwl:id>GAZ:00193866</oboInOwl:id>
        <rdfs:label>Bet She&apos;an National Park</rdfs:label>
    </owl:NamedIndividual>
    


    <!-- http://purl.obolibrary.org/obo/GAZ_00193885 -->

    <owl:NamedIndividual rdf:about="http://purl.obolibrary.org/obo/GAZ_00193885">
        <obo:RO_0001025 rdf:resource="http://purl.obolibrary.org/obo/GAZ_00008742"/>
        <obo:IAO_0000115>A protected area.</obo:IAO_0000115>
        <oboInOwl:hasOBONamespace>GAZ</oboInOwl:hasOBONamespace>
        <oboInOwl:id>GAZ:00193885</oboInOwl:id>
        <rdfs:label>Hurshat Tal National Park</rdfs:label>
    </owl:NamedIndividual>
    


    <!-- http://purl.obolibrary.org/obo/GAZ_00193886 -->

    <owl:NamedIndividual rdf:about="http://purl.obolibrary.org/obo/GAZ_00193886">
        <obo:RO_0001025 rdf:resource="http://purl.obolibrary.org/obo/GAZ_00008742"/>
        <obo:IAO_0000115>A protected area.</obo:IAO_0000115>
        <oboInOwl:hasOBONamespace>GAZ</oboInOwl:hasOBONamespace>
        <oboInOwl:id>GAZ:00193886</oboInOwl:id>
        <rdfs:label>Hula Nature Reserve</rdfs:label>
    </owl:NamedIndividual>
    


    <!-- http://purl.obolibrary.org/obo/GAZ_00193951 -->

    <owl:NamedIndividual rdf:about="http://purl.obolibrary.org/obo/GAZ_00193951">
        <obo:RO_0001025 rdf:resource="http://purl.obolibrary.org/obo/GAZ_00044915"/>
        <obo:IAO_0000115>A large spit of land which now separates the North and the South basins of the Dead Sea. Entirely located in Jordan.</obo:IAO_0000115>
        <oboInOwl:hasOBONamespace>GAZ</oboInOwl:hasOBONamespace>
        <oboInOwl:id>GAZ:00193951</oboInOwl:id>
        <rdfs:label>Lisan Peninsula</rdfs:label>
    </owl:NamedIndividual>
    


    <!-- http://purl.obolibrary.org/obo/GAZ_00230337 -->

    <owl:NamedIndividual rdf:about="http://purl.obolibrary.org/obo/GAZ_00230337">
        <obo:RO_0001025 rdf:resource="http://purl.obolibrary.org/obo/GAZ_00000567"/>
        <oboInOwl:hasOBONamespace>GAZ</oboInOwl:hasOBONamespace>
        <oboInOwl:id>GAZ:00230337</oboInOwl:id>
        <rdfs:label>Sarana River</rdfs:label>
    </owl:NamedIndividual>
    


    <!-- http://purl.obolibrary.org/obo/GAZ_00230338 -->

    <owl:NamedIndividual rdf:about="http://purl.obolibrary.org/obo/GAZ_00230338">
        <obo:RO_0001025 rdf:resource="http://purl.obolibrary.org/obo/GAZ_00000567"/>
        <oboInOwl:hasOBONamespace>GAZ</oboInOwl:hasOBONamespace>
        <oboInOwl:id>GAZ:00230338</oboInOwl:id>
        <rdfs:label>Balasa River</rdfs:label>
    </owl:NamedIndividual>
    


    <!-- http://purl.obolibrary.org/obo/GAZ_00230339 -->

    <owl:NamedIndividual rdf:about="http://purl.obolibrary.org/obo/GAZ_00230339">
        <obo:RO_0001025 rdf:resource="http://purl.obolibrary.org/obo/GAZ_00000567"/>
        <obo:IAO_0000115>A river. A tributary of the Mareb River in Ethiopia.</obo:IAO_0000115>
        <oboInOwl:hasOBONamespace>GAZ</oboInOwl:hasOBONamespace>
        <oboInOwl:id>GAZ:00230339</oboInOwl:id>
        <rdfs:label>Mai Shawesh River</rdfs:label>
    </owl:NamedIndividual>
    


    <!-- http://purl.obolibrary.org/obo/GAZ_00230340 -->

    <owl:NamedIndividual rdf:about="http://purl.obolibrary.org/obo/GAZ_00230340">
        <obo:RO_0001025 rdf:resource="http://purl.obolibrary.org/obo/GAZ_00000567"/>
        <obo:IAO_0000115>A river. A tributary of the Mareb River in Ethiopia.</obo:IAO_0000115>
        <oboInOwl:hasOBONamespace>GAZ</oboInOwl:hasOBONamespace>
        <oboInOwl:id>GAZ:00230340</oboInOwl:id>
        <rdfs:label>&apos;Engweya River</rdfs:label>
    </owl:NamedIndividual>
    


    <!-- http://purl.obolibrary.org/obo/GAZ_00230341 -->

    <owl:NamedIndividual rdf:about="http://purl.obolibrary.org/obo/GAZ_00230341">
        <obo:RO_0001025 rdf:resource="http://purl.obolibrary.org/obo/GAZ_00051205"/>
        <obo:IAO_0000115>A lake. Located in the Northern Red Sea Region, Lake Kulul lies in the Eritrean portion of the Afar Depression.</obo:IAO_0000115>
        <oboInOwl:hasOBONamespace>GAZ</oboInOwl:hasOBONamespace>
        <oboInOwl:id>GAZ:00230341</oboInOwl:id>
        <rdfs:label>Lake Kulul</rdfs:label>
    </owl:NamedIndividual>
    


    <!-- http://purl.obolibrary.org/obo/GAZ_00230359 -->

    <owl:NamedIndividual rdf:about="http://purl.obolibrary.org/obo/GAZ_00230359">
        <obo:IAO_0000115>A paleontogical site. An area in the Middle Awash Valley, in Ethiopia that has provided a rich source of Australopithecines and Homo fossils.</obo:IAO_0000115>
        <oboInOwl:hasOBONamespace>GAZ</oboInOwl:hasOBONamespace>
        <oboInOwl:id>GAZ:00230359</oboInOwl:id>
        <rdfs:label>Bouri Formation</rdfs:label>
    </owl:NamedIndividual>
    


    <!-- http://purl.obolibrary.org/obo/GAZ_00230360 -->

    <owl:NamedIndividual rdf:about="http://purl.obolibrary.org/obo/GAZ_00230360">
        <obo:IAO_0000115>An archaeological site along the Awash River in Ethiopia&apos;s Afar Depression.</obo:IAO_0000115>
        <oboInOwl:hasOBONamespace>GAZ</oboInOwl:hasOBONamespace>
        <oboInOwl:id>GAZ:00230360</oboInOwl:id>
        <rdfs:label>Middle Awash</rdfs:label>
    </owl:NamedIndividual>
    


    <!-- http://purl.obolibrary.org/obo/GAZ_00230365 -->

    <owl:NamedIndividual rdf:about="http://purl.obolibrary.org/obo/GAZ_00230365">
        <obo:RO_0001025 rdf:resource="http://purl.obolibrary.org/obo/GAZ_00052566"/>
        <obo:IAO_0000115>A river of southern Ethiopia. Located inside Omo National Park, it is a tributary of the Omo River.</obo:IAO_0000115>
        <oboInOwl:hasOBONamespace>GAZ</oboInOwl:hasOBONamespace>
        <oboInOwl:id>GAZ:00230365</oboInOwl:id>
        <rdfs:label>Mui River</rdfs:label>
    </owl:NamedIndividual>
    


    <!-- http://purl.obolibrary.org/obo/GAZ_00230367 -->

    <owl:NamedIndividual rdf:about="http://purl.obolibrary.org/obo/GAZ_00230367">
        <obo:RO_0001025 rdf:resource="http://purl.obolibrary.org/obo/GAZ_00076367"/>
        <obo:IAO_0000115>A part of the Mago National Park, W of the Mago River.</obo:IAO_0000115>
        <oboInOwl:hasOBONamespace>GAZ</oboInOwl:hasOBONamespace>
        <oboInOwl:id>GAZ:00230367</oboInOwl:id>
        <rdfs:label>Tama Wildlife Reserve</rdfs:label>
    </owl:NamedIndividual>
    


    <!-- http://purl.obolibrary.org/obo/GAZ_00230368 -->

    <owl:NamedIndividual rdf:about="http://purl.obolibrary.org/obo/GAZ_00230368">
        <obo:RO_0001025 rdf:resource="http://purl.obolibrary.org/obo/GAZ_00076367"/>
        <obo:IAO_0000115>A part of the Mago National Park, E of the Mago River.</obo:IAO_0000115>
        <oboInOwl:hasOBONamespace>GAZ</oboInOwl:hasOBONamespace>
        <oboInOwl:id>GAZ:00230368</oboInOwl:id>
        <rdfs:label>Murle Controlled Hunting Area</rdfs:label>
    </owl:NamedIndividual>
    


    <!-- http://purl.obolibrary.org/obo/GAZ_00230369 -->

    <owl:NamedIndividual rdf:about="http://purl.obolibrary.org/obo/GAZ_00230369">
        <obo:RO_0001025 rdf:resource="http://purl.obolibrary.org/obo/GAZ_00031143"/>
        <obo:IAO_0000115>A river of southern Ethiopia, entirely located in the Debub Omo Zone of the Southern Nations, Nationalities, and People&apos;s Region. It is a tributary of the Omo River.</obo:IAO_0000115>
        <oboInOwl:hasOBONamespace>GAZ</oboInOwl:hasOBONamespace>
        <oboInOwl:id>GAZ:00230369</oboInOwl:id>
        <rdfs:label>Mago River</rdfs:label>
    </owl:NamedIndividual>
    


    <!-- http://purl.obolibrary.org/obo/GAZ_00230372 -->

    <owl:NamedIndividual rdf:about="http://purl.obolibrary.org/obo/GAZ_00230372">
        <obo:IAO_0000115>A hydroelectric dam. Completed 2004.</obo:IAO_0000115>
        <oboInOwl:hasOBONamespace>GAZ</oboInOwl:hasOBONamespace>
        <oboInOwl:id>GAZ:00230372</oboInOwl:id>
        <rdfs:label>Gojeb Dam</rdfs:label>
    </owl:NamedIndividual>
    


    <!-- http://purl.obolibrary.org/obo/GAZ_00230373 -->

    <owl:NamedIndividual rdf:about="http://purl.obolibrary.org/obo/GAZ_00230373">
        <obo:RO_0001025 rdf:resource="http://purl.obolibrary.org/obo/GAZ_00052567"/>
        <obo:IAO_0000115>A river. A tributary of the Omo River.</obo:IAO_0000115>
        <oboInOwl:hasOBONamespace>GAZ</oboInOwl:hasOBONamespace>
        <oboInOwl:id>GAZ:00230373</oboInOwl:id>
        <rdfs:label>Wabi River</rdfs:label>
    </owl:NamedIndividual>
    


    <!-- http://purl.obolibrary.org/obo/GAZ_00230374 -->

    <owl:NamedIndividual rdf:about="http://purl.obolibrary.org/obo/GAZ_00230374">
        <obo:RO_0001025 rdf:resource="http://purl.obolibrary.org/obo/GAZ_00052567"/>
        <obo:IAO_0000115>A hydroelectric dam.</obo:IAO_0000115>
        <oboInOwl:hasOBONamespace>GAZ</oboInOwl:hasOBONamespace>
        <oboInOwl:id>GAZ:00230374</oboInOwl:id>
        <rdfs:label>Gibe III Dam</rdfs:label>
    </owl:NamedIndividual>
    


    <!-- http://purl.obolibrary.org/obo/GAZ_00230375 -->

    <owl:NamedIndividual rdf:about="http://purl.obolibrary.org/obo/GAZ_00230375">
        <obo:IAO_0000115>A hydroelectric dam. Constructed 1986-2004.</obo:IAO_0000115>
        <oboInOwl:hasOBONamespace>GAZ</oboInOwl:hasOBONamespace>
        <oboInOwl:id>GAZ:00230375</oboInOwl:id>
        <rdfs:label>Gilgel Gibe Dam</rdfs:label>
    </owl:NamedIndividual>
    


    <!-- http://purl.obolibrary.org/obo/GAZ_00230376 -->

    <owl:NamedIndividual rdf:about="http://purl.obolibrary.org/obo/GAZ_00230376">
        <obo:RO_0001025 rdf:resource="http://purl.obolibrary.org/obo/GAZ_00052531"/>
        <obo:IAO_0000115>A forest located in Ethiopia within a portion of the Bale Mountains.</obo:IAO_0000115>
        <oboInOwl:hasOBONamespace>GAZ</oboInOwl:hasOBONamespace>
        <oboInOwl:id>GAZ:00230376</oboInOwl:id>
        <rdfs:label>Harenna Forest</rdfs:label>
    </owl:NamedIndividual>
    


    <!-- http://purl.obolibrary.org/obo/GAZ_00230377 -->

    <owl:NamedIndividual rdf:about="http://purl.obolibrary.org/obo/GAZ_00230377">
        <obo:IAO_0000115>A small desert in northern Kenya and southern Ethiopia. The desert is located east of Lake Turkana, the largest permanent desert lake in the world. The settlement of North Horr lies in the desert. Marsabit is the closest major city.</obo:IAO_0000115>
        <oboInOwl:hasOBONamespace>GAZ</oboInOwl:hasOBONamespace>
        <oboInOwl:id>GAZ:00230377</oboInOwl:id>
        <rdfs:label>Chalbi Desert</rdfs:label>
    </owl:NamedIndividual>
    


    <!-- http://purl.obolibrary.org/obo/GAZ_00230382 -->

    <owl:NamedIndividual rdf:about="http://purl.obolibrary.org/obo/GAZ_00230382">
        <obo:RO_0001025 rdf:resource="http://purl.obolibrary.org/obo/GAZ_00000567"/>
        <obo:IAO_0000115>A perennial river in southeastern Ethiopia. Rising in the mountains east of Aleta Wendo, the Dawa flows south and east to join with the Ganale Dorya at the border with Somalia to become the Jubba.</obo:IAO_0000115>
        <oboInOwl:hasOBONamespace>GAZ</oboInOwl:hasOBONamespace>
        <oboInOwl:id>GAZ:00230382</oboInOwl:id>
        <rdfs:label>Dawa River</rdfs:label>
    </owl:NamedIndividual>
    


    <!-- http://purl.obolibrary.org/obo/GAZ_00230394 -->

    <owl:NamedIndividual rdf:about="http://purl.obolibrary.org/obo/GAZ_00230394">
        <obo:RO_0001025 rdf:resource="http://purl.obolibrary.org/obo/GAZ_00031093"/>
        <obo:IAO_0000115>A river of central Ethiopia which, along with the Wanchet River, defined the former district of Marra Biete.</obo:IAO_0000115>
        <oboInOwl:hasOBONamespace>GAZ</oboInOwl:hasOBONamespace>
        <oboInOwl:id>GAZ:00230394</oboInOwl:id>
        <rdfs:label>Adabay River</rdfs:label>
    </owl:NamedIndividual>
    


    <!-- http://purl.obolibrary.org/obo/GAZ_00230398 -->

    <owl:NamedIndividual rdf:about="http://purl.obolibrary.org/obo/GAZ_00230398">
        <obo:RO_0001025 rdf:resource="http://purl.obolibrary.org/obo/GAZ_00031093"/>
        <obo:IAO_0000115>A river. A tributary of the Jamma River. Along with the Adabay River, it defined the border of the former district of Marra Biete.</obo:IAO_0000115>
        <oboInOwl:hasOBONamespace>GAZ</oboInOwl:hasOBONamespace>
        <oboInOwl:id>GAZ:00230398</oboInOwl:id>
        <rdfs:label>Wanchet River</rdfs:label>
    </owl:NamedIndividual>
    


    <!-- http://purl.obolibrary.org/obo/GAZ_00230399 -->

    <owl:NamedIndividual rdf:about="http://purl.obolibrary.org/obo/GAZ_00230399">
        <obo:RO_0001025 rdf:resource="http://purl.obolibrary.org/obo/GAZ_00000567"/>
        <obo:IAO_0000115>A river of central Ethiopia.</obo:IAO_0000115>
        <oboInOwl:hasOBONamespace>GAZ</oboInOwl:hasOBONamespace>
        <oboInOwl:id>GAZ:00230399</oboInOwl:id>
        <rdfs:label>Akaki River</rdfs:label>
    </owl:NamedIndividual>
    


    <!-- http://purl.obolibrary.org/obo/GAZ_00230410 -->

    <owl:NamedIndividual rdf:about="http://purl.obolibrary.org/obo/GAZ_00230410">
        <obo:RO_0001025 rdf:resource="http://purl.obolibrary.org/obo/GAZ_00000567"/>
        <obo:IAO_0000115>A river of southwestern Ethiopia. It is a tributary of the Baro River.</obo:IAO_0000115>
        <oboInOwl:hasOBONamespace>GAZ</oboInOwl:hasOBONamespace>
        <oboInOwl:id>GAZ:00230410</oboInOwl:id>
        <rdfs:label>Jikawo River</rdfs:label>
    </owl:NamedIndividual>
    


    <!-- http://purl.obolibrary.org/obo/GAZ_00230413 -->

    <owl:NamedIndividual rdf:about="http://purl.obolibrary.org/obo/GAZ_00230413">
        <obo:RO_0001025 rdf:resource="http://purl.obolibrary.org/obo/GAZ_00000567"/>
        <obo:IAO_0000115>A river of Ethiopia.</obo:IAO_0000115>
        <oboInOwl:hasOBONamespace>GAZ</oboInOwl:hasOBONamespace>
        <oboInOwl:id>GAZ:00230413</oboInOwl:id>
        <rdfs:label>Alero River</rdfs:label>
    </owl:NamedIndividual>
    


    <!-- http://purl.obolibrary.org/obo/GAZ_00230416 -->

    <owl:NamedIndividual rdf:about="http://purl.obolibrary.org/obo/GAZ_00230416">
        <obo:IAO_0000115>A dam. Constructed 1986.</obo:IAO_0000115>
        <oboInOwl:hasOBONamespace>GAZ</oboInOwl:hasOBONamespace>
        <oboInOwl:id>GAZ:00230416</oboInOwl:id>
        <rdfs:label>Angereb Dam</rdfs:label>
    </owl:NamedIndividual>
    


    <!-- http://purl.obolibrary.org/obo/GAZ_00230418 -->

    <owl:NamedIndividual rdf:about="http://purl.obolibrary.org/obo/GAZ_00230418">
        <obo:RO_0001025 rdf:resource="http://purl.obolibrary.org/obo/GAZ_00000567"/>
        <obo:IAO_0000115>A river of southwestern Ethiopia.</obo:IAO_0000115>
        <oboInOwl:hasOBONamespace>GAZ</oboInOwl:hasOBONamespace>
        <oboInOwl:id>GAZ:00230418</oboInOwl:id>
        <rdfs:label>Awetu River</rdfs:label>
    </owl:NamedIndividual>
    


    <!-- http://purl.obolibrary.org/obo/GAZ_00230419 -->

    <owl:NamedIndividual rdf:about="http://purl.obolibrary.org/obo/GAZ_00230419">
        <obo:RO_0001025 rdf:resource="http://purl.obolibrary.org/obo/GAZ_00000567"/>
        <obo:IAO_0000115>An intermittent river in eastern Ethiopia. Its drainage area is part of the Rift Valley.</obo:IAO_0000115>
        <oboInOwl:hasOBONamespace>GAZ</oboInOwl:hasOBONamespace>
        <oboInOwl:id>GAZ:00230419</oboInOwl:id>
        <rdfs:label>Ayesha River</rdfs:label>
    </owl:NamedIndividual>
    


    <!-- http://purl.obolibrary.org/obo/GAZ_00230429 -->

    <owl:NamedIndividual rdf:about="http://purl.obolibrary.org/obo/GAZ_00230429">
        <obo:RO_0001025 rdf:resource="http://purl.obolibrary.org/obo/GAZ_00000567"/>
        <obo:IAO_0000115>A river of south-central Ethiopia. It rises on the southwestern slopes of Mount Gurage, flowing south along the western side of the Great Rift Valley, to empty into Lake Abaya.</obo:IAO_0000115>
        <oboInOwl:hasOBONamespace>GAZ</oboInOwl:hasOBONamespace>
        <oboInOwl:id>GAZ:00230429</oboInOwl:id>
        <rdfs:label>Bilate River</rdfs:label>
    </owl:NamedIndividual>
    


    <!-- http://purl.obolibrary.org/obo/GAZ_00230430 -->

    <owl:NamedIndividual rdf:about="http://purl.obolibrary.org/obo/GAZ_00230430">
        <obo:RO_0001025 rdf:resource="http://purl.obolibrary.org/obo/GAZ_00000567"/>
        <obo:IAO_0000115>A river of central Ethiopia.</obo:IAO_0000115>
        <oboInOwl:hasOBONamespace>GAZ</oboInOwl:hasOBONamespace>
        <oboInOwl:id>GAZ:00230430</oboInOwl:id>
        <rdfs:label>Cheleleka River</rdfs:label>
    </owl:NamedIndividual>
    


    <!-- http://purl.obolibrary.org/obo/GAZ_00230432 -->

    <owl:NamedIndividual rdf:about="http://purl.obolibrary.org/obo/GAZ_00230432">
        <obo:RO_0001025 rdf:resource="http://purl.obolibrary.org/obo/GAZ_00000567"/>
        <obo:IAO_0000115>A river of eastern Ethiopia. It rises in the Ahmar Mountains to flow north through Dire Dawa towards the Awash River; it is unclear if either its flow or river bed reach that river.</obo:IAO_0000115>
        <oboInOwl:hasOBONamespace>GAZ</oboInOwl:hasOBONamespace>
        <oboInOwl:id>GAZ:00230432</oboInOwl:id>
        <rdfs:label>Dechatu River</rdfs:label>
    </owl:NamedIndividual>
    


    <!-- http://purl.obolibrary.org/obo/GAZ_00230433 -->

    <owl:NamedIndividual rdf:about="http://purl.obolibrary.org/obo/GAZ_00230433">
        <obo:RO_0001025 rdf:resource="http://purl.obolibrary.org/obo/GAZ_00000567"/>
        <obo:IAO_0000115>A river of southwestern Ethiopia.</obo:IAO_0000115>
        <oboInOwl:hasOBONamespace>GAZ</oboInOwl:hasOBONamespace>
        <oboInOwl:id>GAZ:00230433</oboInOwl:id>
        <rdfs:label>Dembi River</rdfs:label>
    </owl:NamedIndividual>
    


    <!-- http://purl.obolibrary.org/obo/GAZ_00230444 -->

    <owl:NamedIndividual rdf:about="http://purl.obolibrary.org/obo/GAZ_00230444">
        <obo:RO_0001025 rdf:resource="http://purl.obolibrary.org/obo/GAZ_00000567"/>
        <obo:IAO_0000115>A river in southwestern Ethiopia.</obo:IAO_0000115>
        <oboInOwl:hasOBONamespace>GAZ</oboInOwl:hasOBONamespace>
        <oboInOwl:id>GAZ:00230444</oboInOwl:id>
        <rdfs:label>Doha River</rdfs:label>
    </owl:NamedIndividual>
    


    <!-- http://purl.obolibrary.org/obo/GAZ_00230445 -->

    <owl:NamedIndividual rdf:about="http://purl.obolibrary.org/obo/GAZ_00230445">
        <obo:RO_0001025 rdf:resource="http://purl.obolibrary.org/obo/GAZ_00000567"/>
        <obo:IAO_0000115>A river of central Ethiopia.</obo:IAO_0000115>
        <oboInOwl:hasOBONamespace>GAZ</oboInOwl:hasOBONamespace>
        <oboInOwl:id>GAZ:00230445</oboInOwl:id>
        <rdfs:label>Dukem River</rdfs:label>
    </owl:NamedIndividual>
    


    <!-- http://purl.obolibrary.org/obo/GAZ_00230452 -->

    <owl:NamedIndividual rdf:about="http://purl.obolibrary.org/obo/GAZ_00230452">
        <obo:RO_0001025 rdf:resource="http://purl.obolibrary.org/obo/GAZ_00000567"/>
        <obo:IAO_0000115>A river of eastern Ethiopia.</obo:IAO_0000115>
        <oboInOwl:hasOBONamespace>GAZ</oboInOwl:hasOBONamespace>
        <oboInOwl:id>GAZ:00230452</oboInOwl:id>
        <rdfs:label>Gololcha River</rdfs:label>
    </owl:NamedIndividual>
    


    <!-- http://purl.obolibrary.org/obo/GAZ_00230455 -->

    <owl:NamedIndividual rdf:about="http://purl.obolibrary.org/obo/GAZ_00230455">
        <obo:RO_0001025 rdf:resource="http://purl.obolibrary.org/obo/GAZ_00000567"/>
        <obo:IAO_0000115>A river of eastern Ethiopia.</obo:IAO_0000115>
        <oboInOwl:hasOBONamespace>GAZ</oboInOwl:hasOBONamespace>
        <oboInOwl:id>GAZ:00230455</oboInOwl:id>
        <rdfs:label>Jerer River</rdfs:label>
    </owl:NamedIndividual>
    


    <!-- http://purl.obolibrary.org/obo/GAZ_00230456 -->

    <owl:NamedIndividual rdf:about="http://purl.obolibrary.org/obo/GAZ_00230456">
        <obo:RO_0001025 rdf:resource="http://purl.obolibrary.org/obo/GAZ_00000567"/>
        <obo:IAO_0000115>A river.</obo:IAO_0000115>
        <oboInOwl:hasOBONamespace>GAZ</oboInOwl:hasOBONamespace>
        <oboInOwl:id>GAZ:00230456</oboInOwl:id>
        <rdfs:label>Kobara River</rdfs:label>
    </owl:NamedIndividual>
    


    <!-- http://purl.obolibrary.org/obo/GAZ_00230458 -->

    <owl:NamedIndividual rdf:about="http://purl.obolibrary.org/obo/GAZ_00230458">
        <obo:RO_0001025 rdf:resource="http://purl.obolibrary.org/obo/GAZ_00000567"/>
        <obo:IAO_0000115>A river of central Ethiopia.</obo:IAO_0000115>
        <oboInOwl:hasOBONamespace>GAZ</oboInOwl:hasOBONamespace>
        <oboInOwl:id>GAZ:00230458</oboInOwl:id>
        <rdfs:label>Keleta River</rdfs:label>
    </owl:NamedIndividual>
    


    <!-- http://purl.obolibrary.org/obo/GAZ_00230461 -->

    <owl:NamedIndividual rdf:about="http://purl.obolibrary.org/obo/GAZ_00230461">
        <obo:RO_0001025 rdf:resource="http://purl.obolibrary.org/obo/GAZ_00000567"/>
        <obo:IAO_0000115>A river of south-central Ethiopia.</obo:IAO_0000115>
        <oboInOwl:hasOBONamespace>GAZ</oboInOwl:hasOBONamespace>
        <oboInOwl:id>GAZ:00230461</oboInOwl:id>
        <rdfs:label>Lagabora River</rdfs:label>
    </owl:NamedIndividual>
    


    <!-- http://purl.obolibrary.org/obo/GAZ_00230462 -->

    <owl:NamedIndividual rdf:about="http://purl.obolibrary.org/obo/GAZ_00230462">
        <obo:RO_0001025 rdf:resource="http://purl.obolibrary.org/obo/GAZ_00000567"/>
        <obo:IAO_0000115>A river of Ethiopia.</obo:IAO_0000115>
        <oboInOwl:hasOBONamespace>GAZ</oboInOwl:hasOBONamespace>
        <oboInOwl:id>GAZ:00230462</oboInOwl:id>
        <rdfs:label>Magyecha River</rdfs:label>
    </owl:NamedIndividual>
    


    <!-- http://purl.obolibrary.org/obo/GAZ_00230463 -->

    <owl:NamedIndividual rdf:about="http://purl.obolibrary.org/obo/GAZ_00230463">
        <obo:RO_0001025 rdf:resource="http://purl.obolibrary.org/obo/GAZ_00000567"/>
        <obo:IAO_0000115>A river in central Ethiopia. It empties into Lake Zway.</obo:IAO_0000115>
        <oboInOwl:hasOBONamespace>GAZ</oboInOwl:hasOBONamespace>
        <oboInOwl:id>GAZ:00230463</oboInOwl:id>
        <rdfs:label>Meki River</rdfs:label>
    </owl:NamedIndividual>
    


    <!-- http://purl.obolibrary.org/obo/GAZ_00230465 -->

    <owl:NamedIndividual rdf:about="http://purl.obolibrary.org/obo/GAZ_00230465">
        <obo:RO_0001025 rdf:resource="http://purl.obolibrary.org/obo/GAZ_00000567"/>
        <obo:IAO_0000115>A river of central Ethiopia. Tributaries include the Wedecha and Belbela.</obo:IAO_0000115>
        <oboInOwl:hasOBONamespace>GAZ</oboInOwl:hasOBONamespace>
        <oboInOwl:id>GAZ:00230465</oboInOwl:id>
        <rdfs:label>Modjo River</rdfs:label>
    </owl:NamedIndividual>
    


    <!-- http://purl.obolibrary.org/obo/GAZ_00230475 -->

    <owl:NamedIndividual rdf:about="http://purl.obolibrary.org/obo/GAZ_00230475">
        <obo:RO_0001025 rdf:resource="http://purl.obolibrary.org/obo/GAZ_00000567"/>
        <obo:IAO_0000115>A river of southwestern Ethiopia.</obo:IAO_0000115>
        <oboInOwl:hasOBONamespace>GAZ</oboInOwl:hasOBONamespace>
        <oboInOwl:id>GAZ:00230475</oboInOwl:id>
        <rdfs:label>Sor River</rdfs:label>
    </owl:NamedIndividual>
    


    <!-- http://purl.obolibrary.org/obo/GAZ_00233536 -->

    <owl:NamedIndividual rdf:about="http://purl.obolibrary.org/obo/GAZ_00233536">
        <obo:IAO_0000115>A dam on the Blue Nile near the town of Sennar, Sudan. Constructed 1925.</obo:IAO_0000115>
        <oboInOwl:hasOBONamespace>GAZ</oboInOwl:hasOBONamespace>
        <oboInOwl:id>GAZ:00233536</oboInOwl:id>
        <rdfs:label>Sennar Dam</rdfs:label>
    </owl:NamedIndividual>
    


    <!-- http://purl.obolibrary.org/obo/GAZ_00233537 -->

    <owl:NamedIndividual rdf:about="http://purl.obolibrary.org/obo/GAZ_00233537">
        <obo:IAO_0000115>A hydroelectric dam. Impounds El Roseires Lake. Completed 1966.</obo:IAO_0000115>
        <oboInOwl:hasOBONamespace>GAZ</oboInOwl:hasOBONamespace>
        <oboInOwl:id>GAZ:00233537</oboInOwl:id>
        <rdfs:label>El Roseires Dam</rdfs:label>
    </owl:NamedIndividual>
    


    <!-- http://purl.obolibrary.org/obo/GAZ_00234085 -->

    <owl:NamedIndividual rdf:about="http://purl.obolibrary.org/obo/GAZ_00234085">
        <obo:IAO_0000115>A hydroelectric dam. Located at the Ruzizi River outlet from Lake Kivu. Constructed 1958.</obo:IAO_0000115>
        <oboInOwl:hasOBONamespace>GAZ</oboInOwl:hasOBONamespace>
        <oboInOwl:id>GAZ:00234085</oboInOwl:id>
        <rdfs:label>Ruzizi I Hydroelectric Dam</rdfs:label>
    </owl:NamedIndividual>
    


    <!-- http://purl.obolibrary.org/obo/GAZ_00234089 -->

    <owl:NamedIndividual rdf:about="http://purl.obolibrary.org/obo/GAZ_00234089">
        <obo:IAO_0000115>Water falls.</obo:IAO_0000115>
        <oboInOwl:hasOBONamespace>GAZ</oboInOwl:hasOBONamespace>
        <oboInOwl:id>GAZ:00234089</oboInOwl:id>
        <rdfs:label>Chutes de la Kagera</rdfs:label>
    </owl:NamedIndividual>
    


    <!-- http://purl.obolibrary.org/obo/GAZ_00235791 -->

    <owl:NamedIndividual rdf:about="http://purl.obolibrary.org/obo/GAZ_00235791">
        <obo:IAO_0000115>A river. A tributary of the Kagera River.</obo:IAO_0000115>
        <oboInOwl:hasOBONamespace>GAZ</oboInOwl:hasOBONamespace>
        <oboInOwl:id>GAZ:00235791</oboInOwl:id>
        <rdfs:label>Muvumba River</rdfs:label>
    </owl:NamedIndividual>
    


    <!-- http://purl.obolibrary.org/obo/GAZ_00235792 -->

    <owl:NamedIndividual rdf:about="http://purl.obolibrary.org/obo/GAZ_00235792">
        <oboInOwl:hasOBONamespace>GAZ</oboInOwl:hasOBONamespace>
        <oboInOwl:id>GAZ:00235792</oboInOwl:id>
        <rdfs:label>Karangaza River</rdfs:label>
    </owl:NamedIndividual>
    


    <!-- http://purl.obolibrary.org/obo/GAZ_00235793 -->

    <owl:NamedIndividual rdf:about="http://purl.obolibrary.org/obo/GAZ_00235793">
        <oboInOwl:hasOBONamespace>GAZ</oboInOwl:hasOBONamespace>
        <oboInOwl:id>GAZ:00235793</oboInOwl:id>
        <rdfs:label>Kamiramugezi River</rdfs:label>
    </owl:NamedIndividual>
    


    <!-- http://purl.obolibrary.org/obo/GAZ_00235795 -->

    <owl:NamedIndividual rdf:about="http://purl.obolibrary.org/obo/GAZ_00235795">
        <obo:IAO_0000115>A river flowing into Lake Kivu.</obo:IAO_0000115>
        <oboInOwl:hasOBONamespace>GAZ</oboInOwl:hasOBONamespace>
        <oboInOwl:id>GAZ:00235795</oboInOwl:id>
        <rdfs:label>Kalundura River</rdfs:label>
    </owl:NamedIndividual>
    


    <!-- http://purl.obolibrary.org/obo/GAZ_00236097 -->

    <owl:NamedIndividual rdf:about="http://purl.obolibrary.org/obo/GAZ_00236097">
        <obo:RO_0001025 rdf:resource="http://purl.obolibrary.org/obo/GAZ_00000007"/>
        <obo:IAO_0000115>An arid part of the Great Rift Valley in Kenya, directly south of Lake Turkana. The valley is floored by a seasonal stream complex, the Suguta River, that terminates in the seasonal playa Lake Alablab. Lake Logipi, a saline, alkaline lake lies at the northern end of the valley, where it is separated from Lake Turkana by a complex series of volcanoes called the Barrier.</obo:IAO_0000115>
        <oboInOwl:hasOBONamespace>GAZ</oboInOwl:hasOBONamespace>
        <oboInOwl:id>GAZ:00236097</oboInOwl:id>
        <rdfs:label>Suguta Valley</rdfs:label>
    </owl:NamedIndividual>
    


    <!-- http://purl.obolibrary.org/obo/GAZ_00236098 -->

    <owl:NamedIndividual rdf:about="http://purl.obolibrary.org/obo/GAZ_00236098">
        <obo:RO_0001025 rdf:resource="http://purl.obolibrary.org/obo/GAZ_00236097"/>
        <obo:IAO_0000115>A seasonal playa lake.</obo:IAO_0000115>
        <oboInOwl:hasOBONamespace>GAZ</oboInOwl:hasOBONamespace>
        <oboInOwl:id>GAZ:00236098</oboInOwl:id>
        <rdfs:label>Lake Alablab</rdfs:label>
    </owl:NamedIndividual>
    


    <!-- http://purl.obolibrary.org/obo/GAZ_00236099 -->

    <owl:NamedIndividual rdf:about="http://purl.obolibrary.org/obo/GAZ_00236099">
        <obo:RO_0001025 rdf:resource="http://purl.obolibrary.org/obo/GAZ_00236097"/>
        <obo:IAO_0000115>An intermittent river.</obo:IAO_0000115>
        <oboInOwl:hasOBONamespace>GAZ</oboInOwl:hasOBONamespace>
        <oboInOwl:id>GAZ:00236099</oboInOwl:id>
        <rdfs:label>Suguta River</rdfs:label>
    </owl:NamedIndividual>
    


    <!-- http://purl.obolibrary.org/obo/GAZ_00236105 -->

    <owl:NamedIndividual rdf:about="http://purl.obolibrary.org/obo/GAZ_00236105">
        <obo:RO_0001025 rdf:resource="http://purl.obolibrary.org/obo/GAZ_00000007"/>
        <obo:IAO_0000115>A fault-scarp caused by to post-Miocene faulting and there are Miocene beds visible. The escarpment is part of the western wall of the Great Rift Valley.</obo:IAO_0000115>
        <oboInOwl:hasOBONamespace>GAZ</oboInOwl:hasOBONamespace>
        <oboInOwl:id>GAZ:00236105</oboInOwl:id>
        <rdfs:label>Elgeyo Escarpment</rdfs:label>
    </owl:NamedIndividual>
    


    <!-- http://purl.obolibrary.org/obo/GAZ_00236116 -->

    <owl:NamedIndividual rdf:about="http://purl.obolibrary.org/obo/GAZ_00236116">
        <obo:RO_0001025 rdf:resource="http://purl.obolibrary.org/obo/GAZ_00000007"/>
        <obo:IAO_0000115>Peaks in a ridge along the Great Rift Valley, located southwest near Nairobi, in southern Kenya.</obo:IAO_0000115>
        <oboInOwl:hasOBONamespace>GAZ</oboInOwl:hasOBONamespace>
        <oboInOwl:id>GAZ:00236116</oboInOwl:id>
        <rdfs:label>Ngong Hills</rdfs:label>
    </owl:NamedIndividual>
    


    <!-- http://purl.obolibrary.org/obo/GAZ_00236121 -->

    <owl:NamedIndividual rdf:about="http://purl.obolibrary.org/obo/GAZ_00236121">
        <rdf:type rdf:resource="http://purl.obolibrary.org/obo/ENVO_00000100"/>
        <rdf:type rdf:resource="http://purl.obolibrary.org/obo/ENVO_00000479"/>
        <obo:RO_0001025 rdf:resource="http://purl.obolibrary.org/obo/GAZ_00076405"/>
        <obo:IAO_0000115>A gorge. A former outlet of Lake Naivasha.</obo:IAO_0000115>
        <oboInOwl:hasOBONamespace>GAZ</oboInOwl:hasOBONamespace>
        <oboInOwl:id>GAZ:00236121</oboInOwl:id>
        <rdfs:label>Njorowa Gorge</rdfs:label>
    </owl:NamedIndividual>
    


    <!-- http://purl.obolibrary.org/obo/GAZ_00236122 -->

    <owl:NamedIndividual rdf:about="http://purl.obolibrary.org/obo/GAZ_00236122">
        <obo:RO_0001025 rdf:resource="http://purl.obolibrary.org/obo/GAZ_00000007"/>
        <obo:IAO_0000115>A highland area of lush green rolling hills at the edge of the Great Rift Valley in the Rift Valley Province of Kenya.</obo:IAO_0000115>
        <oboInOwl:hasOBONamespace>GAZ</oboInOwl:hasOBONamespace>
        <oboInOwl:id>GAZ:00236122</oboInOwl:id>
        <rdfs:label>Nandi Hills</rdfs:label>
    </owl:NamedIndividual>
    


    <!-- http://purl.obolibrary.org/obo/GAZ_00236170 -->

    <owl:NamedIndividual rdf:about="http://purl.obolibrary.org/obo/GAZ_00236170">
        <obo:RO_0001025 rdf:resource="http://purl.obolibrary.org/obo/GAZ_00052895"/>
        <obo:IAO_0000115>A bay.</obo:IAO_0000115>
        <oboInOwl:hasOBONamespace>GAZ</oboInOwl:hasOBONamespace>
        <oboInOwl:id>GAZ:00236170</oboInOwl:id>
        <rdfs:label>Naya Bay</rdfs:label>
    </owl:NamedIndividual>
    


    <!-- http://purl.obolibrary.org/obo/GAZ_00236171 -->

    <owl:NamedIndividual rdf:about="http://purl.obolibrary.org/obo/GAZ_00236171">
        <obo:RO_0001025 rdf:resource="http://purl.obolibrary.org/obo/GAZ_00052895"/>
        <obo:IAO_0000115>A bay.</obo:IAO_0000115>
        <oboInOwl:hasOBONamespace>GAZ</oboInOwl:hasOBONamespace>
        <oboInOwl:id>GAZ:00236171</oboInOwl:id>
        <rdfs:label>Nyakach Bay</rdfs:label>
    </owl:NamedIndividual>
    


    <!-- http://purl.obolibrary.org/obo/GAZ_00236172 -->

    <owl:NamedIndividual rdf:about="http://purl.obolibrary.org/obo/GAZ_00236172">
        <obo:RO_0001025 rdf:resource="http://purl.obolibrary.org/obo/GAZ_00052895"/>
        <obo:IAO_0000115>A bay.</obo:IAO_0000115>
        <oboInOwl:hasOBONamespace>GAZ</oboInOwl:hasOBONamespace>
        <oboInOwl:id>GAZ:00236172</oboInOwl:id>
        <rdfs:label>Osodo Bay</rdfs:label>
    </owl:NamedIndividual>
    


    <!-- http://purl.obolibrary.org/obo/GAZ_00236173 -->

    <owl:NamedIndividual rdf:about="http://purl.obolibrary.org/obo/GAZ_00236173">
        <obo:RO_0001025 rdf:resource="http://purl.obolibrary.org/obo/GAZ_00052895"/>
        <obo:IAO_0000115>A bay.</obo:IAO_0000115>
        <oboInOwl:hasOBONamespace>GAZ</oboInOwl:hasOBONamespace>
        <oboInOwl:id>GAZ:00236173</oboInOwl:id>
        <rdfs:label>Kendu Bay</rdfs:label>
    </owl:NamedIndividual>
    


    <!-- http://purl.obolibrary.org/obo/GAZ_00236174 -->

    <owl:NamedIndividual rdf:about="http://purl.obolibrary.org/obo/GAZ_00236174">
        <obo:RO_0001025 rdf:resource="http://purl.obolibrary.org/obo/GAZ_00052895"/>
        <obo:IAO_0000115>A bay.</obo:IAO_0000115>
        <oboInOwl:hasOBONamespace>GAZ</oboInOwl:hasOBONamespace>
        <oboInOwl:id>GAZ:00236174</oboInOwl:id>
        <rdfs:label>Ruri Bay</rdfs:label>
    </owl:NamedIndividual>
    


    <!-- http://purl.obolibrary.org/obo/GAZ_00236175 -->

    <owl:NamedIndividual rdf:about="http://purl.obolibrary.org/obo/GAZ_00236175">
        <obo:RO_0001025 rdf:resource="http://purl.obolibrary.org/obo/GAZ_00052895"/>
        <obo:IAO_0000115>A bay.</obo:IAO_0000115>
        <oboInOwl:hasOBONamespace>GAZ</oboInOwl:hasOBONamespace>
        <oboInOwl:id>GAZ:00236175</oboInOwl:id>
        <rdfs:label>Mirunda Bay</rdfs:label>
    </owl:NamedIndividual>
    


    <!-- http://purl.obolibrary.org/obo/GAZ_00236176 -->

    <owl:NamedIndividual rdf:about="http://purl.obolibrary.org/obo/GAZ_00236176">
        <obo:RO_0001025 rdf:resource="http://purl.obolibrary.org/obo/GAZ_00052895"/>
        <obo:IAO_0000115>A bay.</obo:IAO_0000115>
        <oboInOwl:hasOBONamespace>GAZ</oboInOwl:hasOBONamespace>
        <oboInOwl:id>GAZ:00236176</oboInOwl:id>
        <rdfs:label>Olambwe Bay</rdfs:label>
    </owl:NamedIndividual>
    


    <!-- http://purl.obolibrary.org/obo/GAZ_00236183 -->

    <owl:NamedIndividual rdf:about="http://purl.obolibrary.org/obo/GAZ_00236183">
        <obo:RO_0001025 rdf:resource="http://purl.obolibrary.org/obo/GAZ_00008411"/>
        <obo:IAO_0000115>An alkaline hot spring running into Lake Bogoria.</obo:IAO_0000115>
        <oboInOwl:hasOBONamespace>GAZ</oboInOwl:hasOBONamespace>
        <oboInOwl:id>GAZ:00236183</oboInOwl:id>
        <rdfs:label>Loburu</rdfs:label>
    </owl:NamedIndividual>
    


    <!-- http://purl.obolibrary.org/obo/GAZ_00236184 -->

    <owl:NamedIndividual rdf:about="http://purl.obolibrary.org/obo/GAZ_00236184">
        <obo:RO_0001025 rdf:resource="http://purl.obolibrary.org/obo/GAZ_00008411"/>
        <obo:IAO_0000115>An alkaline hot spring running into Lake Bogoria.</obo:IAO_0000115>
        <oboInOwl:hasOBONamespace>GAZ</oboInOwl:hasOBONamespace>
        <oboInOwl:id>GAZ:00236184</oboInOwl:id>
        <rdfs:label>Chemurkeu</rdfs:label>
    </owl:NamedIndividual>
    


    <!-- http://purl.obolibrary.org/obo/GAZ_00236185 -->

    <owl:NamedIndividual rdf:about="http://purl.obolibrary.org/obo/GAZ_00236185">
        <obo:RO_0001025 rdf:resource="http://purl.obolibrary.org/obo/GAZ_00008411"/>
        <obo:IAO_0000115>A group of alkaline hot spring running into Lake Bogoria.</obo:IAO_0000115>
        <oboInOwl:hasOBONamespace>GAZ</oboInOwl:hasOBONamespace>
        <oboInOwl:id>GAZ:00236185</oboInOwl:id>
        <rdfs:label>Southern group of hot springs</rdfs:label>
    </owl:NamedIndividual>
    


    <!-- http://purl.obolibrary.org/obo/GAZ_00236186 -->

    <owl:NamedIndividual rdf:about="http://purl.obolibrary.org/obo/GAZ_00236186">
        <obo:RO_0001025 rdf:resource="http://purl.obolibrary.org/obo/GAZ_00236185"/>
        <obo:IAO_0000115>An alkaline hot spring running into Lake Bogoria.</obo:IAO_0000115>
        <oboInOwl:hasOBONamespace>GAZ</oboInOwl:hasOBONamespace>
        <oboInOwl:id>GAZ:00236186</oboInOwl:id>
        <rdfs:label>Ng&apos;wasis</rdfs:label>
    </owl:NamedIndividual>
    


    <!-- http://purl.obolibrary.org/obo/GAZ_00236187 -->

    <owl:NamedIndividual rdf:about="http://purl.obolibrary.org/obo/GAZ_00236187">
        <obo:RO_0001025 rdf:resource="http://purl.obolibrary.org/obo/GAZ_00236185"/>
        <obo:IAO_0000115>An alkaline hot spring running into Lake Bogoria.</obo:IAO_0000115>
        <oboInOwl:hasOBONamespace>GAZ</oboInOwl:hasOBONamespace>
        <oboInOwl:id>GAZ:00236187</oboInOwl:id>
        <rdfs:label>Koibobei</rdfs:label>
    </owl:NamedIndividual>
    


    <!-- http://purl.obolibrary.org/obo/GAZ_00236188 -->

    <owl:NamedIndividual rdf:about="http://purl.obolibrary.org/obo/GAZ_00236188">
        <obo:RO_0001025 rdf:resource="http://purl.obolibrary.org/obo/GAZ_00236185"/>
        <obo:IAO_0000115>An alkaline hot spring running into Lake Bogoria.</obo:IAO_0000115>
        <oboInOwl:hasOBONamespace>GAZ</oboInOwl:hasOBONamespace>
        <oboInOwl:id>GAZ:00236188</oboInOwl:id>
        <rdfs:label>Losaramat</rdfs:label>
    </owl:NamedIndividual>
    


    <!-- http://purl.obolibrary.org/obo/GAZ_00236192 -->

    <owl:NamedIndividual rdf:about="http://purl.obolibrary.org/obo/GAZ_00236192">
        <obo:RO_0001025 rdf:resource="http://purl.obolibrary.org/obo/GAZ_00000007"/>
        <obo:IAO_0000115>An escarpment in southern Kenya. The escarpment is around 50 km long and elongated in N-W direction. Its northern edge approximately 120 km southwest of Nairobi, while the southern edge is near the Tanzanian border, at the northwestern corner of Lake Natron. The southern Ewaso Ngiro river flows along the foot of the escarpment, while Loita Hills are located west of the escarpment . The escarpment forms the western wall of the Great Rift Valley.</obo:IAO_0000115>
        <oboInOwl:hasOBONamespace>GAZ</oboInOwl:hasOBONamespace>
        <oboInOwl:id>GAZ:00236192</oboInOwl:id>
        <rdfs:label>Nguruman Escarpment</rdfs:label>
    </owl:NamedIndividual>
    


    <!-- http://purl.obolibrary.org/obo/GAZ_00236193 -->

    <owl:NamedIndividual rdf:about="http://purl.obolibrary.org/obo/GAZ_00236193">
        <obo:RO_0001025 rdf:resource="http://purl.obolibrary.org/obo/GAZ_00236192"/>
        <obo:IAO_0000115>A protected area.</obo:IAO_0000115>
        <oboInOwl:hasOBONamespace>GAZ</oboInOwl:hasOBONamespace>
        <oboInOwl:id>GAZ:00236193</oboInOwl:id>
        <rdfs:label>Shompole Conservancy</rdfs:label>
    </owl:NamedIndividual>
    


    <!-- http://purl.obolibrary.org/obo/GAZ_00236194 -->

    <owl:NamedIndividual rdf:about="http://purl.obolibrary.org/obo/GAZ_00236194">
        <obo:IAO_0000115>A river in Rift Valley Province, Kenya. It flows northward into Lake Turkana.</obo:IAO_0000115>
        <oboInOwl:hasOBONamespace>GAZ</oboInOwl:hasOBONamespace>
        <oboInOwl:id>GAZ:00236194</oboInOwl:id>
        <rdfs:label>Kerio River</rdfs:label>
    </owl:NamedIndividual>
    


    <!-- http://purl.obolibrary.org/obo/GAZ_00236202 -->

    <owl:NamedIndividual rdf:about="http://purl.obolibrary.org/obo/GAZ_00236202">
        <obo:IAO_0000115>A hydroelectric plant.</obo:IAO_0000115>
        <oboInOwl:hasOBONamespace>GAZ</oboInOwl:hasOBONamespace>
        <oboInOwl:id>GAZ:00236202</oboInOwl:id>
        <rdfs:label>Turkwel Hydro Power Plant</rdfs:label>
    </owl:NamedIndividual>
    


    <!-- http://purl.obolibrary.org/obo/GAZ_00236239 -->

    <owl:NamedIndividual rdf:about="http://purl.obolibrary.org/obo/GAZ_00236239">
        <obo:RO_0001025 rdf:resource="http://purl.obolibrary.org/obo/GAZ_00136138"/>
        <obo:IAO_0000115>A lake.</obo:IAO_0000115>
        <oboInOwl:hasOBONamespace>GAZ</oboInOwl:hasOBONamespace>
        <oboInOwl:id>GAZ:00236239</oboInOwl:id>
        <rdfs:label>Lake Kitangiri</rdfs:label>
    </owl:NamedIndividual>
    


    <!-- http://purl.obolibrary.org/obo/GAZ_00236354 -->

    <owl:NamedIndividual rdf:about="http://purl.obolibrary.org/obo/GAZ_00236354">
        <obo:RO_0001025 rdf:resource="http://purl.obolibrary.org/obo/GAZ_00015452"/>
        <obo:IAO_0000115>An island in Lake Victoria claimed by both Uganda and Kenya.</obo:IAO_0000115>
        <oboInOwl:hasOBONamespace>GAZ</oboInOwl:hasOBONamespace>
        <oboInOwl:id>GAZ:00236354</oboInOwl:id>
        <rdfs:label>Migingo Island</rdfs:label>
    </owl:NamedIndividual>
    


    <!-- http://purl.obolibrary.org/obo/GAZ_00236355 -->

    <owl:NamedIndividual rdf:about="http://purl.obolibrary.org/obo/GAZ_00236355">
        <obo:RO_0001025 rdf:resource="http://purl.obolibrary.org/obo/GAZ_00015452"/>
        <obo:IAO_0000115>A Kenyan island whose westerly most point was used to demarcate the border between Kenya and Uganda just after parallel 1 degree in Lake Victoria.</obo:IAO_0000115>
        <oboInOwl:hasOBONamespace>GAZ</oboInOwl:hasOBONamespace>
        <oboInOwl:id>GAZ:00236355</oboInOwl:id>
        <rdfs:label>Pyramid Island</rdfs:label>
    </owl:NamedIndividual>
    


    <!-- http://purl.obolibrary.org/obo/GAZ_00236356 -->

    <owl:NamedIndividual rdf:about="http://purl.obolibrary.org/obo/GAZ_00236356">
        <obo:RO_0001025 rdf:resource="http://purl.obolibrary.org/obo/GAZ_00015452"/>
        <obo:IAO_0000115>An island.</obo:IAO_0000115>
        <oboInOwl:hasOBONamespace>GAZ</oboInOwl:hasOBONamespace>
        <oboInOwl:id>GAZ:00236356</oboInOwl:id>
        <rdfs:label>Ilemba island</rdfs:label>
    </owl:NamedIndividual>
    


    <!-- http://purl.obolibrary.org/obo/GAZ_00236357 -->

    <owl:NamedIndividual rdf:about="http://purl.obolibrary.org/obo/GAZ_00236357">
        <obo:RO_0001025 rdf:resource="http://purl.obolibrary.org/obo/GAZ_00015452"/>
        <obo:IAO_0000115>An island.</obo:IAO_0000115>
        <oboInOwl:hasOBONamespace>GAZ</oboInOwl:hasOBONamespace>
        <oboInOwl:id>GAZ:00236357</oboInOwl:id>
        <rdfs:label>Sumba Island</rdfs:label>
    </owl:NamedIndividual>
    


    <!-- http://purl.obolibrary.org/obo/GAZ_00236358 -->

    <owl:NamedIndividual rdf:about="http://purl.obolibrary.org/obo/GAZ_00236358">
        <obo:RO_0001025 rdf:resource="http://purl.obolibrary.org/obo/GAZ_00015452"/>
        <obo:IAO_0000115>An island in Lake Victoria.</obo:IAO_0000115>
        <oboInOwl:hasOBONamespace>GAZ</oboInOwl:hasOBONamespace>
        <oboInOwl:id>GAZ:00236358</oboInOwl:id>
        <rdfs:label>Mageta Island</rdfs:label>
    </owl:NamedIndividual>
    


    <!-- http://purl.obolibrary.org/obo/GAZ_00236359 -->

    <owl:NamedIndividual rdf:about="http://purl.obolibrary.org/obo/GAZ_00236359">
        <obo:RO_0001025 rdf:resource="http://purl.obolibrary.org/obo/GAZ_00015452"/>
        <obo:IAO_0000115>An island.</obo:IAO_0000115>
        <oboInOwl:hasOBONamespace>GAZ</oboInOwl:hasOBONamespace>
        <oboInOwl:id>GAZ:00236359</oboInOwl:id>
        <rdfs:label>Kiringiti Island</rdfs:label>
    </owl:NamedIndividual>
    


    <!-- http://purl.obolibrary.org/obo/GAZ_00236360 -->

    <owl:NamedIndividual rdf:about="http://purl.obolibrary.org/obo/GAZ_00236360">
        <obo:RO_0001025 rdf:resource="http://purl.obolibrary.org/obo/GAZ_00015452"/>
        <obo:IAO_0000115>An island.</obo:IAO_0000115>
        <oboInOwl:hasOBONamespace>GAZ</oboInOwl:hasOBONamespace>
        <oboInOwl:id>GAZ:00236360</oboInOwl:id>
        <rdfs:label>Sigulu Island</rdfs:label>
    </owl:NamedIndividual>
    


    <!-- http://purl.obolibrary.org/obo/GAZ_00236361 -->

    <owl:NamedIndividual rdf:about="http://purl.obolibrary.org/obo/GAZ_00236361">
        <obo:RO_0001025 rdf:resource="http://purl.obolibrary.org/obo/GAZ_00015452"/>
        <obo:IAO_0000115>An island.</obo:IAO_0000115>
        <oboInOwl:hasOBONamespace>GAZ</oboInOwl:hasOBONamespace>
        <oboInOwl:id>GAZ:00236361</oboInOwl:id>
        <rdfs:label>Seguti Island</rdfs:label>
    </owl:NamedIndividual>
    


    <!-- http://purl.obolibrary.org/obo/GAZ_00236362 -->

    <owl:NamedIndividual rdf:about="http://purl.obolibrary.org/obo/GAZ_00236362">
        <obo:RO_0001025 rdf:resource="http://purl.obolibrary.org/obo/GAZ_00015452"/>
        <obo:IAO_0000115>An island.</obo:IAO_0000115>
        <oboInOwl:hasOBONamespace>GAZ</oboInOwl:hasOBONamespace>
        <oboInOwl:id>GAZ:00236362</oboInOwl:id>
        <rdfs:label>Dagusi Island</rdfs:label>
    </owl:NamedIndividual>
    


    <!-- http://purl.obolibrary.org/obo/GAZ_00236363 -->

    <owl:NamedIndividual rdf:about="http://purl.obolibrary.org/obo/GAZ_00236363">
        <obo:RO_0001025 rdf:resource="http://purl.obolibrary.org/obo/GAZ_00015452"/>
        <obo:IAO_0000115>An island.</obo:IAO_0000115>
        <oboInOwl:hasOBONamespace>GAZ</oboInOwl:hasOBONamespace>
        <oboInOwl:id>GAZ:00236363</oboInOwl:id>
        <rdfs:label>Vumba Island</rdfs:label>
    </owl:NamedIndividual>
    


    <!-- http://purl.obolibrary.org/obo/GAZ_00236364 -->

    <owl:NamedIndividual rdf:about="http://purl.obolibrary.org/obo/GAZ_00236364">
        <obo:RO_0001025 rdf:resource="http://purl.obolibrary.org/obo/GAZ_00015452"/>
        <obo:IAO_0000115>An island.</obo:IAO_0000115>
        <oboInOwl:hasOBONamespace>GAZ</oboInOwl:hasOBONamespace>
        <oboInOwl:id>GAZ:00236364</oboInOwl:id>
        <rdfs:label>Kaza Island</rdfs:label>
    </owl:NamedIndividual>
    


    <!-- http://purl.obolibrary.org/obo/GAZ_00236365 -->

    <owl:NamedIndividual rdf:about="http://purl.obolibrary.org/obo/GAZ_00236365">
        <obo:RO_0001025 rdf:resource="http://purl.obolibrary.org/obo/GAZ_00015452"/>
        <obo:IAO_0000115>An island.</obo:IAO_0000115>
        <oboInOwl:hasOBONamespace>GAZ</oboInOwl:hasOBONamespace>
        <oboInOwl:id>GAZ:00236365</oboInOwl:id>
        <rdfs:label>Nambuga Island</rdfs:label>
    </owl:NamedIndividual>
    


    <!-- http://purl.obolibrary.org/obo/GAZ_00236366 -->

    <owl:NamedIndividual rdf:about="http://purl.obolibrary.org/obo/GAZ_00236366">
        <obo:RO_0001025 rdf:resource="http://purl.obolibrary.org/obo/GAZ_00015452"/>
        <obo:IAO_0000115>An island.</obo:IAO_0000115>
        <oboInOwl:hasOBONamespace>GAZ</oboInOwl:hasOBONamespace>
        <oboInOwl:id>GAZ:00236366</oboInOwl:id>
        <rdfs:label>Simu Island</rdfs:label>
    </owl:NamedIndividual>
    


    <!-- http://purl.obolibrary.org/obo/GAZ_00236597 -->

    <owl:NamedIndividual rdf:about="http://purl.obolibrary.org/obo/GAZ_00236597">
        <obo:RO_0001025 rdf:resource="http://purl.obolibrary.org/obo/GAZ_00040046"/>
        <obo:IAO_0000115>An island.</obo:IAO_0000115>
        <oboInOwl:hasOBONamespace>GAZ</oboInOwl:hasOBONamespace>
        <oboInOwl:id>GAZ:00236597</oboInOwl:id>
        <rdfs:label>Ngamba Island</rdfs:label>
    </owl:NamedIndividual>
    


    <!-- http://purl.obolibrary.org/obo/GAZ_00236598 -->

    <owl:NamedIndividual rdf:about="http://purl.obolibrary.org/obo/GAZ_00236598">
        <obo:RO_0001025 rdf:resource="http://purl.obolibrary.org/obo/GAZ_00040046"/>
        <obo:IAO_0000115>An island.</obo:IAO_0000115>
        <oboInOwl:hasOBONamespace>GAZ</oboInOwl:hasOBONamespace>
        <oboInOwl:id>GAZ:00236598</oboInOwl:id>
        <rdfs:label>Nsadzi Island</rdfs:label>
    </owl:NamedIndividual>
    


    <!-- http://purl.obolibrary.org/obo/GAZ_00236599 -->

    <owl:NamedIndividual rdf:about="http://purl.obolibrary.org/obo/GAZ_00236599">
        <obo:RO_0001025 rdf:resource="http://purl.obolibrary.org/obo/GAZ_00040046"/>
        <obo:IAO_0000115>An island.</obo:IAO_0000115>
        <oboInOwl:hasOBONamespace>GAZ</oboInOwl:hasOBONamespace>
        <oboInOwl:id>GAZ:00236599</oboInOwl:id>
        <rdfs:label>Bulago Island</rdfs:label>
    </owl:NamedIndividual>
    


    <!-- http://purl.obolibrary.org/obo/GAZ_00237137 -->

    <owl:NamedIndividual rdf:about="http://purl.obolibrary.org/obo/GAZ_00237137">
        <obo:IAO_0000115>A wide, 32 km long body of water that links Lake Edward and Lake George, and a dominant feature of Queen Elizabeth National Park.</obo:IAO_0000115>
        <oboInOwl:hasOBONamespace>GAZ</oboInOwl:hasOBONamespace>
        <oboInOwl:id>GAZ:00237137</oboInOwl:id>
        <rdfs:label>Kazinga Channel</rdfs:label>
    </owl:NamedIndividual>
    


    <!-- http://purl.obolibrary.org/obo/GAZ_00237174 -->

    <owl:NamedIndividual rdf:about="http://purl.obolibrary.org/obo/GAZ_00237174">
        <obo:IAO_0000115>A hydroelectric power station across the White Nile near to its source at Lake Victoria in Uganda.</obo:IAO_0000115>
        <oboInOwl:hasOBONamespace>GAZ</oboInOwl:hasOBONamespace>
        <oboInOwl:id>GAZ:00237174</oboInOwl:id>
        <rdfs:label>Nalubaale Power Station</rdfs:label>
    </owl:NamedIndividual>
    


    <!-- http://purl.obolibrary.org/obo/GAZ_00237175 -->

    <owl:NamedIndividual rdf:about="http://purl.obolibrary.org/obo/GAZ_00237175">
        <obo:IAO_0000115>A hydroelectric power station located in Jinja, Jinja District, in eastern central Uganda.</obo:IAO_0000115>
        <oboInOwl:hasOBONamespace>GAZ</oboInOwl:hasOBONamespace>
        <oboInOwl:id>GAZ:00237175</oboInOwl:id>
        <rdfs:label>Kiira Power Station</rdfs:label>
    </owl:NamedIndividual>
    


    <!-- http://purl.obolibrary.org/obo/GAZ_00237176 -->

    <owl:NamedIndividual rdf:about="http://purl.obolibrary.org/obo/GAZ_00237176">
        <obo:IAO_0000115>A hydroelectric power project located at the headwaters of River Nile, about 16 km north of Jinja at the former location of Bujagali Falls.</obo:IAO_0000115>
        <oboInOwl:hasOBONamespace>GAZ</oboInOwl:hasOBONamespace>
        <oboInOwl:id>GAZ:00237176</oboInOwl:id>
        <rdfs:label>Bujagali Power Station</rdfs:label>
    </owl:NamedIndividual>
    


    <!-- http://purl.obolibrary.org/obo/GAZ_00237412 -->

    <owl:NamedIndividual rdf:about="http://purl.obolibrary.org/obo/GAZ_00237412">
        <obo:IAO_0000115>A river of eastern Uganda in eastern Africa. It flows in a southern and south-westerly direction and eventually via the Okere River reaches Lake Kyoga.</obo:IAO_0000115>
        <oboInOwl:hasOBONamespace>GAZ</oboInOwl:hasOBONamespace>
        <oboInOwl:id>GAZ:00237412</oboInOwl:id>
        <rdfs:label>Okot River</rdfs:label>
    </owl:NamedIndividual>
    


    <!-- http://purl.obolibrary.org/obo/GAZ_00237449 -->

    <owl:NamedIndividual rdf:about="http://purl.obolibrary.org/obo/GAZ_00237449">
        <obo:IAO_0000115>A river.</obo:IAO_0000115>
        <oboInOwl:hasOBONamespace>GAZ</oboInOwl:hasOBONamespace>
        <oboInOwl:id>GAZ:00237449</oboInOwl:id>
        <rdfs:label>Lufubu River</rdfs:label>
    </owl:NamedIndividual>
    


    <!-- http://purl.obolibrary.org/obo/GAZ_00240890 -->

    <owl:NamedIndividual rdf:about="http://purl.obolibrary.org/obo/GAZ_00240890">
        <obo:RO_0001025 rdf:resource="http://purl.obolibrary.org/obo/GAZ_00008558"/>
        <obo:IAO_0000115>An island.</obo:IAO_0000115>
        <oboInOwl:hasOBONamespace>GAZ</oboInOwl:hasOBONamespace>
        <oboInOwl:id>GAZ:00240890</oboInOwl:id>
        <rdfs:label>Ile Wahu</rdfs:label>
    </owl:NamedIndividual>
    


    <!-- http://purl.obolibrary.org/obo/GAZ_00240891 -->

    <owl:NamedIndividual rdf:about="http://purl.obolibrary.org/obo/GAZ_00240891">
        <obo:RO_0001025 rdf:resource="http://purl.obolibrary.org/obo/GAZ_00008558"/>
        <obo:IAO_0000115>An island.</obo:IAO_0000115>
        <oboInOwl:hasOBONamespace>GAZ</oboInOwl:hasOBONamespace>
        <oboInOwl:id>GAZ:00240891</oboInOwl:id>
        <rdfs:label>Ile Bugarura</rdfs:label>
    </owl:NamedIndividual>
    


    <!-- http://purl.obolibrary.org/obo/GAZ_00240892 -->

    <owl:NamedIndividual rdf:about="http://purl.obolibrary.org/obo/GAZ_00240892">
        <obo:RO_0001025 rdf:resource="http://purl.obolibrary.org/obo/GAZ_00008558"/>
        <obo:IAO_0000115>An island.</obo:IAO_0000115>
        <oboInOwl:hasOBONamespace>GAZ</oboInOwl:hasOBONamespace>
        <oboInOwl:id>GAZ:00240892</oboInOwl:id>
        <rdfs:label>Ile Gombe</rdfs:label>
    </owl:NamedIndividual>
    


    <!-- http://purl.obolibrary.org/obo/GAZ_00247089 -->

    <owl:NamedIndividual rdf:about="http://purl.obolibrary.org/obo/GAZ_00247089">
        <obo:IAO_0000115>A river. A tributary of the Ruvyironza River.</obo:IAO_0000115>
        <oboInOwl:hasOBONamespace>GAZ</oboInOwl:hasOBONamespace>
        <oboInOwl:id>GAZ:00247089</oboInOwl:id>
        <rdfs:label>Karuzi River</rdfs:label>
    </owl:NamedIndividual>
    


    <!-- http://purl.obolibrary.org/obo/GAZ_00247090 -->

    <owl:NamedIndividual rdf:about="http://purl.obolibrary.org/obo/GAZ_00247090">
        <obo:IAO_0000115>A river. It rises in the far east of Burundi, close to the Tanzanian border, and flows southwestwards, anti-parallel with the Rurubu for 48 km, before turning abruptly northwards to a confluence with the Rurubu.</obo:IAO_0000115>
        <oboInOwl:hasOBONamespace>GAZ</oboInOwl:hasOBONamespace>
        <oboInOwl:id>GAZ:00247090</oboInOwl:id>
        <rdfs:label>Kayongozi River</rdfs:label>
    </owl:NamedIndividual>
    


    <!-- http://purl.obolibrary.org/obo/GAZ_00247094 -->

    <owl:NamedIndividual rdf:about="http://purl.obolibrary.org/obo/GAZ_00247094">
        <obo:IAO_0000115>A river that flows into Lake Tanganyika in the south of Burundi.</obo:IAO_0000115>
        <oboInOwl:hasOBONamespace>GAZ</oboInOwl:hasOBONamespace>
        <oboInOwl:id>GAZ:00247094</oboInOwl:id>
        <rdfs:label>Mugwezi River</rdfs:label>
    </owl:NamedIndividual>
    


    <!-- http://purl.obolibrary.org/obo/GAZ_00247095 -->

    <owl:NamedIndividual rdf:about="http://purl.obolibrary.org/obo/GAZ_00247095">
        <obo:IAO_0000115>A river that flows into Lake Tanganyika in the south of Burundi.</obo:IAO_0000115>
        <oboInOwl:hasOBONamespace>GAZ</oboInOwl:hasOBONamespace>
        <oboInOwl:id>GAZ:00247095</oboInOwl:id>
        <rdfs:label>Luaba River</rdfs:label>
    </owl:NamedIndividual>
    


    <!-- http://purl.obolibrary.org/obo/GAZ_00248119 -->

    <owl:NamedIndividual rdf:about="http://purl.obolibrary.org/obo/GAZ_00248119">
        <obo:RO_0001025 rdf:resource="http://purl.obolibrary.org/obo/GAZ_00052532"/>
        <obo:IAO_0000115>A freshwater lake.</obo:IAO_0000115>
        <oboInOwl:hasOBONamespace>GAZ</oboInOwl:hasOBONamespace>
        <oboInOwl:id>GAZ:00248119</oboInOwl:id>
        <rdfs:label>Garba Gurastch Lake</rdfs:label>
    </owl:NamedIndividual>
    


    <!-- http://purl.obolibrary.org/obo/GAZ_00248120 -->

    <owl:NamedIndividual rdf:about="http://purl.obolibrary.org/obo/GAZ_00248120">
        <obo:RO_0001025 rdf:resource="http://purl.obolibrary.org/obo/GAZ_00052532"/>
        <obo:IAO_0000115>A freshwater lake.</obo:IAO_0000115>
        <oboInOwl:hasOBONamespace>GAZ</oboInOwl:hasOBONamespace>
        <oboInOwl:id>GAZ:00248120</oboInOwl:id>
        <rdfs:label>Hora Orgona Lake</rdfs:label>
    </owl:NamedIndividual>
    


    <!-- http://purl.obolibrary.org/obo/GAZ_00248121 -->

    <owl:NamedIndividual rdf:about="http://purl.obolibrary.org/obo/GAZ_00248121">
        <obo:RO_0001025 rdf:resource="http://purl.obolibrary.org/obo/GAZ_00053656"/>
        <obo:IAO_0000115>An alkaline crater lake.</obo:IAO_0000115>
        <oboInOwl:hasOBONamespace>GAZ</oboInOwl:hasOBONamespace>
        <oboInOwl:id>GAZ:00248121</oboInOwl:id>
        <rdfs:label>Lake Biete Mengest</rdfs:label>
    </owl:NamedIndividual>
    


    <!-- http://purl.obolibrary.org/obo/GAZ_00248122 -->

    <owl:NamedIndividual rdf:about="http://purl.obolibrary.org/obo/GAZ_00248122">
        <obo:RO_0001025 rdf:resource="http://purl.obolibrary.org/obo/GAZ_00053656"/>
        <obo:IAO_0000115>An alkaline crater lake.</obo:IAO_0000115>
        <oboInOwl:hasOBONamespace>GAZ</oboInOwl:hasOBONamespace>
        <oboInOwl:id>GAZ:00248122</oboInOwl:id>
        <rdfs:label>Lake Bishoftu</rdfs:label>
    </owl:NamedIndividual>
    


    <!-- http://purl.obolibrary.org/obo/GAZ_00248123 -->

    <owl:NamedIndividual rdf:about="http://purl.obolibrary.org/obo/GAZ_00248123">
        <obo:RO_0001025 rdf:resource="http://purl.obolibrary.org/obo/GAZ_00053656"/>
        <obo:IAO_0000115>An alkaline crater lake.</obo:IAO_0000115>
        <oboInOwl:hasOBONamespace>GAZ</oboInOwl:hasOBONamespace>
        <oboInOwl:id>GAZ:00248123</oboInOwl:id>
        <rdfs:label>Lake Pawlo</rdfs:label>
    </owl:NamedIndividual>
    


    <!-- http://purl.obolibrary.org/obo/GAZ_00248124 -->

    <owl:NamedIndividual rdf:about="http://purl.obolibrary.org/obo/GAZ_00248124">
        <obo:RO_0001025 rdf:resource="http://purl.obolibrary.org/obo/GAZ_00053656"/>
        <obo:IAO_0000115>An alkaline crater lake.</obo:IAO_0000115>
        <oboInOwl:hasOBONamespace>GAZ</oboInOwl:hasOBONamespace>
        <oboInOwl:id>GAZ:00248124</oboInOwl:id>
        <rdfs:label>Lake Aranguadi</rdfs:label>
    </owl:NamedIndividual>
    


    <!-- http://purl.obolibrary.org/obo/GAZ_00248125 -->

    <owl:NamedIndividual rdf:about="http://purl.obolibrary.org/obo/GAZ_00248125">
        <obo:RO_0001025 rdf:resource="http://purl.obolibrary.org/obo/GAZ_00053656"/>
        <obo:IAO_0000115>An alkaline crater lake.</obo:IAO_0000115>
        <oboInOwl:hasOBONamespace>GAZ</oboInOwl:hasOBONamespace>
        <oboInOwl:id>GAZ:00248125</oboInOwl:id>
        <rdfs:label>Lake Kilotes</rdfs:label>
    </owl:NamedIndividual>
    


    <!-- http://purl.obolibrary.org/obo/GAZ_00248126 -->

    <owl:NamedIndividual rdf:about="http://purl.obolibrary.org/obo/GAZ_00248126">
        <rdf:type rdf:resource="http://purl.obolibrary.org/obo/ENVO_00000309"/>
        <obo:RO_0001025 rdf:resource="http://purl.obolibrary.org/obo/GAZ_00000007"/>
        <obo:IAO_0000115>A pan.</obo:IAO_0000115>
        <oboInOwl:hasOBONamespace>GAZ</oboInOwl:hasOBONamespace>
        <oboInOwl:id>GAZ:00248126</oboInOwl:id>
        <rdfs:label>Ch&apos;ew Bahir</rdfs:label>
    </owl:NamedIndividual>
    


    <!-- http://purl.obolibrary.org/obo/GAZ_00248131 -->

    <owl:NamedIndividual rdf:about="http://purl.obolibrary.org/obo/GAZ_00248131">
        <obo:RO_0001025 rdf:resource="http://purl.obolibrary.org/obo/GAZ_00000784"/>
        <obo:IAO_0000115>A river.</obo:IAO_0000115>
        <oboInOwl:hasOBONamespace>GAZ</oboInOwl:hasOBONamespace>
        <oboInOwl:id>GAZ:00248131</oboInOwl:id>
        <rdfs:label>Gelana Shet&apos;</rdfs:label>
    </owl:NamedIndividual>
    


    <!-- http://purl.obolibrary.org/obo/GAZ_00248132 -->

    <owl:NamedIndividual rdf:about="http://purl.obolibrary.org/obo/GAZ_00248132">
        <obo:RO_0001025 rdf:resource="http://purl.obolibrary.org/obo/GAZ_00000779"/>
        <obo:IAO_0000115>A crater lake.</obo:IAO_0000115>
        <oboInOwl:hasOBONamespace>GAZ</oboInOwl:hasOBONamespace>
        <oboInOwl:id>GAZ:00248132</oboInOwl:id>
        <rdfs:label>Beda Hayk&apos;</rdfs:label>
    </owl:NamedIndividual>
    


    <!-- http://purl.obolibrary.org/obo/GAZ_00248133 -->

    <owl:NamedIndividual rdf:about="http://purl.obolibrary.org/obo/GAZ_00248133">
        <obo:RO_0001025 rdf:resource="http://purl.obolibrary.org/obo/GAZ_00000779"/>
        <obo:IAO_0000115>A lake located in the permanent swamp above Lake Yardi.</obo:IAO_0000115>
        <oboInOwl:hasOBONamespace>GAZ</oboInOwl:hasOBONamespace>
        <oboInOwl:id>GAZ:00248133</oboInOwl:id>
        <rdfs:label>Lake Kaddabasa</rdfs:label>
    </owl:NamedIndividual>
    


    <!-- http://purl.obolibrary.org/obo/GAZ_00248134 -->

    <owl:NamedIndividual rdf:about="http://purl.obolibrary.org/obo/GAZ_00248134">
        <obo:RO_0001025 rdf:resource="http://purl.obolibrary.org/obo/GAZ_00000779"/>
        <obo:IAO_0000115>A wetland. Towards the end of these swamps the Awash branches into eastern and western channels.</obo:IAO_0000115>
        <oboInOwl:hasOBONamespace>GAZ</oboInOwl:hasOBONamespace>
        <oboInOwl:id>GAZ:00248134</oboInOwl:id>
        <rdfs:label>Dubti Swamps</rdfs:label>
    </owl:NamedIndividual>
    


    <!-- http://purl.obolibrary.org/obo/GAZ_00248136 -->

    <owl:NamedIndividual rdf:about="http://purl.obolibrary.org/obo/GAZ_00248136">
        <obo:RO_0001025 rdf:resource="http://purl.obolibrary.org/obo/GAZ_00051205"/>
        <obo:IAO_0000115>A saline lake.</obo:IAO_0000115>
        <oboInOwl:hasOBONamespace>GAZ</oboInOwl:hasOBONamespace>
        <oboInOwl:id>GAZ:00248136</oboInOwl:id>
        <rdfs:label>Lake Asale</rdfs:label>
    </owl:NamedIndividual>
    


    <!-- http://purl.obolibrary.org/obo/GAZ_00248137 -->

    <owl:NamedIndividual rdf:about="http://purl.obolibrary.org/obo/GAZ_00248137">
        <obo:IAO_0000115>A reservoir in Ethiopia. Constructed 1960.</obo:IAO_0000115>
        <oboInOwl:hasOBONamespace>GAZ</oboInOwl:hasOBONamespace>
        <oboInOwl:id>GAZ:00248137</oboInOwl:id>
        <rdfs:label>Zula Lake</rdfs:label>
    </owl:NamedIndividual>
    


    <!-- http://purl.obolibrary.org/obo/GAZ_00248138 -->

    <owl:NamedIndividual rdf:about="http://purl.obolibrary.org/obo/GAZ_00248138">
        <obo:RO_0001025 rdf:resource="http://purl.obolibrary.org/obo/GAZ_00000567"/>
        <obo:IAO_0000115>A wetland located near Butajira high in the Western Highlands above Lake Ziway in the Rift Valley, to which they drain via the Me&apos;ki River.</obo:IAO_0000115>
        <oboInOwl:hasOBONamespace>GAZ</oboInOwl:hasOBONamespace>
        <oboInOwl:id>GAZ:00248138</oboInOwl:id>
        <rdfs:label>Tufta Swamps</rdfs:label>
    </owl:NamedIndividual>
    


    <!-- http://purl.obolibrary.org/obo/GAZ_00251586 -->

    <owl:NamedIndividual rdf:about="http://purl.obolibrary.org/obo/GAZ_00251586">
        <obo:IAO_0000115>A river that rises in the hills southwest of Irbid city and drains west into the Jordan Valley, entering the Jordan River about 20 km south of Lake Tiberias.</obo:IAO_0000115>
        <oboInOwl:hasOBONamespace>GAZ</oboInOwl:hasOBONamespace>
        <oboInOwl:id>GAZ:00251586</oboInOwl:id>
        <rdfs:label>Wadi Ziglab</rdfs:label>
    </owl:NamedIndividual>
    


    <!-- http://purl.obolibrary.org/obo/GAZ_00251587 -->

    <owl:NamedIndividual rdf:about="http://purl.obolibrary.org/obo/GAZ_00251587">
        <obo:IAO_0000115>A dam. Located about 15 km south-southwest of Ajlun.</obo:IAO_0000115>
        <oboInOwl:hasOBONamespace>GAZ</oboInOwl:hasOBONamespace>
        <oboInOwl:id>GAZ:00251587</oboInOwl:id>
        <rdfs:label>KingTalal Dam</rdfs:label>
    </owl:NamedIndividual>
    


    <!-- http://purl.obolibrary.org/obo/GAZ_00251592 -->

    <owl:NamedIndividual rdf:about="http://purl.obolibrary.org/obo/GAZ_00251592">
        <obo:IAO_0000115>A dam.</obo:IAO_0000115>
        <oboInOwl:hasOBONamespace>GAZ</oboInOwl:hasOBONamespace>
        <oboInOwl:id>GAZ:00251592</oboInOwl:id>
        <rdfs:label>Kafrein Dam</rdfs:label>
    </owl:NamedIndividual>
    


    <!-- http://purl.obolibrary.org/obo/GAZ_00251593 -->

    <owl:NamedIndividual rdf:about="http://purl.obolibrary.org/obo/GAZ_00251593">
        <obo:IAO_0000115>A dam.</obo:IAO_0000115>
        <oboInOwl:hasOBONamespace>GAZ</oboInOwl:hasOBONamespace>
        <oboInOwl:id>GAZ:00251593</oboInOwl:id>
        <rdfs:label>Shu&apos;eib Dam</rdfs:label>
    </owl:NamedIndividual>
    


    <!-- http://purl.obolibrary.org/obo/GAZ_00251594 -->

    <owl:NamedIndividual rdf:about="http://purl.obolibrary.org/obo/GAZ_00251594">
        <obo:RO_0001025 rdf:resource="http://purl.obolibrary.org/obo/GAZ_00044915"/>
        <obo:IAO_0000115>A saline lake.</obo:IAO_0000115>
        <oboInOwl:hasOBONamespace>GAZ</oboInOwl:hasOBONamespace>
        <oboInOwl:id>GAZ:00251594</oboInOwl:id>
        <rdfs:label>Kibed Pool</rdfs:label>
    </owl:NamedIndividual>
    


    <!-- http://purl.obolibrary.org/obo/GAZ_00251595 -->

    <owl:NamedIndividual rdf:about="http://purl.obolibrary.org/obo/GAZ_00251595">
        <obo:IAO_0000115>A wadi. It enters Wadi Mujib from the north only a few km from the shores of the Dead Sea.</obo:IAO_0000115>
        <oboInOwl:hasOBONamespace>GAZ</oboInOwl:hasOBONamespace>
        <oboInOwl:id>GAZ:00251595</oboInOwl:id>
        <rdfs:label>Wadi Hidan</rdfs:label>
    </owl:NamedIndividual>
    


    <!-- http://purl.obolibrary.org/obo/GAZ_00251642 -->

    <owl:NamedIndividual rdf:about="http://purl.obolibrary.org/obo/GAZ_00251642">
        <obo:RO_0001025 rdf:resource="http://purl.obolibrary.org/obo/GAZ_00041537"/>
        <obo:IAO_0000115>A part of Lake Naivasha. It becomes a discrete, but contiguous, basin at low water.</obo:IAO_0000115>
        <oboInOwl:hasOBONamespace>GAZ</oboInOwl:hasOBONamespace>
        <oboInOwl:id>GAZ:00251642</oboInOwl:id>
        <rdfs:label>Lake Oloidien</rdfs:label>
    </owl:NamedIndividual>
    


    <!-- http://purl.obolibrary.org/obo/GAZ_00251652 -->

    <owl:NamedIndividual rdf:about="http://purl.obolibrary.org/obo/GAZ_00251652">
        <obo:RO_0001025 rdf:resource="http://purl.obolibrary.org/obo/GAZ_00000007"/>
        <obo:IAO_0000115>A lake. It is situated on the Nyandarua Plateau at the foot of the Aberdare Mountains.</obo:IAO_0000115>
        <oboInOwl:hasOBONamespace>GAZ</oboInOwl:hasOBONamespace>
        <oboInOwl:id>GAZ:00251652</oboInOwl:id>
        <rdfs:label>Lake Ilpolosat</rdfs:label>
    </owl:NamedIndividual>
    


    <!-- http://purl.obolibrary.org/obo/GAZ_00251653 -->

    <owl:NamedIndividual rdf:about="http://purl.obolibrary.org/obo/GAZ_00251653">
        <obo:IAO_0000115>A river.</obo:IAO_0000115>
        <oboInOwl:hasOBONamespace>GAZ</oboInOwl:hasOBONamespace>
        <oboInOwl:id>GAZ:00251653</oboInOwl:id>
        <rdfs:label>Malewa River</rdfs:label>
    </owl:NamedIndividual>
    


    <!-- http://purl.obolibrary.org/obo/GAZ_00251816 -->

    <owl:NamedIndividual rdf:about="http://purl.obolibrary.org/obo/GAZ_00251816">
        <obo:RO_0001025 rdf:resource="http://purl.obolibrary.org/obo/GAZ_00044906"/>
        <obo:IAO_0000115>A wetland. Located in the western Beka&apos;a Valley south of the main Beirut to Damascus highway, 10 km south-southwest of Qabb Elias town and about 35 km southeast of Beirut.</obo:IAO_0000115>
        <oboInOwl:hasOBONamespace>GAZ</oboInOwl:hasOBONamespace>
        <oboInOwl:id>GAZ:00251816</oboInOwl:id>
        <rdfs:label>Ainmiq Swamp</rdfs:label>
    </owl:NamedIndividual>
    


    <!-- http://purl.obolibrary.org/obo/GAZ_00251903 -->

    <owl:NamedIndividual rdf:about="http://purl.obolibrary.org/obo/GAZ_00251903">
        <obo:IAO_0000115>A widening of the Shire River?</obo:IAO_0000115>
        <oboInOwl:hasOBONamespace>GAZ</oboInOwl:hasOBONamespace>
        <oboInOwl:id>GAZ:00251903</oboInOwl:id>
        <rdfs:label>Bangula Lagoon</rdfs:label>
    </owl:NamedIndividual>
    


    <!-- http://purl.obolibrary.org/obo/GAZ_00251905 -->

    <owl:NamedIndividual rdf:about="http://purl.obolibrary.org/obo/GAZ_00251905">
        <obo:RO_0001025 rdf:resource="http://purl.obolibrary.org/obo/GAZ_00041528"/>
        <obo:IAO_0000115>An island.</obo:IAO_0000115>
        <oboInOwl:hasOBONamespace>GAZ</oboInOwl:hasOBONamespace>
        <oboInOwl:id>GAZ:00251905</oboInOwl:id>
        <rdfs:label>Nchisi Island</rdfs:label>
    </owl:NamedIndividual>
    


    <!-- http://purl.obolibrary.org/obo/GAZ_00255602 -->

    <owl:NamedIndividual rdf:about="http://purl.obolibrary.org/obo/GAZ_00255602">
        <obo:IAO_0000115>A river that carries the overspill from Lake Muhazi.</obo:IAO_0000115>
        <oboInOwl:hasOBONamespace>GAZ</oboInOwl:hasOBONamespace>
        <oboInOwl:id>GAZ:00255602</oboInOwl:id>
        <rdfs:label>Nyabugogo River</rdfs:label>
    </owl:NamedIndividual>
    


    <!-- http://purl.obolibrary.org/obo/GAZ_00256482 -->

    <owl:NamedIndividual rdf:about="http://purl.obolibrary.org/obo/GAZ_00256482">
        <obo:IAO_0000115>An artificial lake. Impounded by El Roseires Dam.</obo:IAO_0000115>
        <oboInOwl:hasOBONamespace>GAZ</oboInOwl:hasOBONamespace>
        <oboInOwl:id>GAZ:00256482</oboInOwl:id>
        <rdfs:label>El Roseires Lake</rdfs:label>
    </owl:NamedIndividual>
    


    <!-- http://purl.obolibrary.org/obo/GAZ_00256483 -->

    <owl:NamedIndividual rdf:about="http://purl.obolibrary.org/obo/GAZ_00256483">
        <obo:IAO_0000115>An artifiical lake. Impounded by Sennar Dam.</obo:IAO_0000115>
        <oboInOwl:hasOBONamespace>GAZ</oboInOwl:hasOBONamespace>
        <oboInOwl:id>GAZ:00256483</oboInOwl:id>
        <rdfs:label>Sennar Lake</rdfs:label>
    </owl:NamedIndividual>
    


    <!-- http://purl.obolibrary.org/obo/GAZ_00256484 -->

    <owl:NamedIndividual rdf:about="http://purl.obolibrary.org/obo/GAZ_00256484">
        <obo:IAO_0000115>A dam. Impounds Kashim el Girlba Lake. Completed 1964.</obo:IAO_0000115>
        <oboInOwl:hasOBONamespace>GAZ</oboInOwl:hasOBONamespace>
        <oboInOwl:id>GAZ:00256484</oboInOwl:id>
        <rdfs:label>Kashim el Girlba Dam</rdfs:label>
    </owl:NamedIndividual>
    


    <!-- http://purl.obolibrary.org/obo/GAZ_00256485 -->

    <owl:NamedIndividual rdf:about="http://purl.obolibrary.org/obo/GAZ_00256485">
        <obo:IAO_0000115>An artifiical lake. Impounded by Kashim el Girlba Dam. Completed 1964.</obo:IAO_0000115>
        <oboInOwl:hasOBONamespace>GAZ</oboInOwl:hasOBONamespace>
        <oboInOwl:id>GAZ:00256485</oboInOwl:id>
        <rdfs:label>Kashim el Girlba Lake</rdfs:label>
    </owl:NamedIndividual>
    


    <!-- http://purl.obolibrary.org/obo/GAZ_00256741 -->

    <owl:NamedIndividual rdf:about="http://purl.obolibrary.org/obo/GAZ_00256741">
        <obo:IAO_0000115>A river.</obo:IAO_0000115>
        <oboInOwl:hasOBONamespace>GAZ</oboInOwl:hasOBONamespace>
        <oboInOwl:id>GAZ:00256741</oboInOwl:id>
        <rdfs:label>Ziuwe River</rdfs:label>
    </owl:NamedIndividual>
    


    <!-- http://purl.obolibrary.org/obo/GAZ_00256743 -->

    <owl:NamedIndividual rdf:about="http://purl.obolibrary.org/obo/GAZ_00256743">
        <obo:RO_0001025 rdf:resource="http://purl.obolibrary.org/obo/GAZ_00256741"/>
        <obo:IAO_0000115>A lake.</obo:IAO_0000115>
        <oboInOwl:hasOBONamespace>GAZ</oboInOwl:hasOBONamespace>
        <oboInOwl:id>GAZ:00256743</oboInOwl:id>
        <rdfs:label>Lake Sagara</rdfs:label>
    </owl:NamedIndividual>
    


    <!-- http://purl.obolibrary.org/obo/GAZ_00260236 -->

    <owl:NamedIndividual rdf:about="http://purl.obolibrary.org/obo/GAZ_00260236">
        <obo:RO_0001025 rdf:resource="http://purl.obolibrary.org/obo/GAZ_00015452"/>
        <obo:IAO_0000115>An island. S of Vumba Island.</obo:IAO_0000115>
        <oboInOwl:hasOBONamespace>GAZ</oboInOwl:hasOBONamespace>
        <oboInOwl:id>GAZ:00260236</oboInOwl:id>
        <rdfs:label>Sagitu Island</rdfs:label>
    </owl:NamedIndividual>
    


    <!-- http://purl.obolibrary.org/obo/GAZ_00260237 -->

    <owl:NamedIndividual rdf:about="http://purl.obolibrary.org/obo/GAZ_00260237">
        <obo:RO_0001025 rdf:resource="http://purl.obolibrary.org/obo/GAZ_00015452"/>
        <obo:IAO_0000115>A bay.</obo:IAO_0000115>
        <oboInOwl:hasOBONamespace>GAZ</oboInOwl:hasOBONamespace>
        <oboInOwl:id>GAZ:00260237</oboInOwl:id>
        <rdfs:label>Sango Bay</rdfs:label>
    </owl:NamedIndividual>
    


    <!-- http://purl.obolibrary.org/obo/GAZ_00260238 -->

    <owl:NamedIndividual rdf:about="http://purl.obolibrary.org/obo/GAZ_00260238">
        <obo:RO_0001025 rdf:resource="http://purl.obolibrary.org/obo/GAZ_00015452"/>
        <obo:IAO_0000115>A channel N of Bugala Island.</obo:IAO_0000115>
        <oboInOwl:hasOBONamespace>GAZ</oboInOwl:hasOBONamespace>
        <oboInOwl:id>GAZ:00260238</oboInOwl:id>
        <rdfs:label>Salisbury Channel</rdfs:label>
    </owl:NamedIndividual>
    


    <!-- http://purl.obolibrary.org/obo/GAZ_00260292 -->

    <owl:NamedIndividual rdf:about="http://purl.obolibrary.org/obo/GAZ_00260292">
        <rdf:type rdf:resource="http://purl.obolibrary.org/obo/ENVO_00000475"/>
        <obo:RO_0001025 rdf:resource="http://purl.obolibrary.org/obo/GAZ_00058791"/>
        <obo:IAO_0000115>An arm of Lake Kyoga.</obo:IAO_0000115>
        <oboInOwl:hasOBONamespace>GAZ</oboInOwl:hasOBONamespace>
        <oboInOwl:id>GAZ:00260292</oboInOwl:id>
        <rdfs:label>Mpologoma Arm</rdfs:label>
    </owl:NamedIndividual>
    


    <!-- http://purl.obolibrary.org/obo/GAZ_00260963 -->

    <owl:NamedIndividual rdf:about="http://purl.obolibrary.org/obo/GAZ_00260963">
        <obo:RO_0001025 rdf:resource="http://purl.obolibrary.org/obo/GAZ_00041530"/>
        <obo:IAO_0000115>An island.</obo:IAO_0000115>
        <oboInOwl:hasOBONamespace>GAZ</oboInOwl:hasOBONamespace>
        <oboInOwl:id>GAZ:00260963</oboInOwl:id>
        <rdfs:label>N&apos;Kole Island</rdfs:label>
    </owl:NamedIndividual>
    


    <!-- http://purl.obolibrary.org/obo/GAZ_00260964 -->

    <owl:NamedIndividual rdf:about="http://purl.obolibrary.org/obo/GAZ_00260964">
        <obo:RO_0001025 rdf:resource="http://purl.obolibrary.org/obo/GAZ_00058782"/>
        <obo:IAO_0000115>A lake lagoon in Zambia. It is in the Luapula River swamps south of Lake Mweru, in the Luapula Province of Zambia.</obo:IAO_0000115>
        <oboInOwl:hasOBONamespace>GAZ</oboInOwl:hasOBONamespace>
        <oboInOwl:id>GAZ:00260964</oboInOwl:id>
        <rdfs:label>Pembe Lagoon</rdfs:label>
    </owl:NamedIndividual>
    


    <!-- http://purl.obolibrary.org/obo/GAZ_00260965 -->

    <owl:NamedIndividual rdf:about="http://purl.obolibrary.org/obo/GAZ_00260965">
        <obo:RO_0001025 rdf:resource="http://purl.obolibrary.org/obo/GAZ_00058782"/>
        <obo:IAO_0000115>A lake on the Luapula Floodplain.</obo:IAO_0000115>
        <oboInOwl:hasOBONamespace>GAZ</oboInOwl:hasOBONamespace>
        <oboInOwl:id>GAZ:00260965</oboInOwl:id>
        <rdfs:label>Lake Kuswa</rdfs:label>
    </owl:NamedIndividual>
    


    <!-- http://purl.obolibrary.org/obo/GAZ_00260966 -->

    <owl:NamedIndividual rdf:about="http://purl.obolibrary.org/obo/GAZ_00260966">
        <obo:RO_0001025 rdf:resource="http://purl.obolibrary.org/obo/GAZ_00058782"/>
        <obo:IAO_0000115>A lake on the Luapula Floodplain.</obo:IAO_0000115>
        <oboInOwl:hasOBONamespace>GAZ</oboInOwl:hasOBONamespace>
        <oboInOwl:id>GAZ:00260966</oboInOwl:id>
        <rdfs:label>Lake Kitshomponshi</rdfs:label>
    </owl:NamedIndividual>
    


    <!-- http://purl.obolibrary.org/obo/GAZ_00260967 -->

    <owl:NamedIndividual rdf:about="http://purl.obolibrary.org/obo/GAZ_00260967">
        <obo:RO_0001025 rdf:resource="http://purl.obolibrary.org/obo/GAZ_00058782"/>
        <obo:IAO_0000115>A lake on the Luapula Floodplain.</obo:IAO_0000115>
        <oboInOwl:hasOBONamespace>GAZ</oboInOwl:hasOBONamespace>
        <oboInOwl:id>GAZ:00260967</oboInOwl:id>
        <rdfs:label>Lake Kifukula</rdfs:label>
    </owl:NamedIndividual>
    


    <!-- http://purl.obolibrary.org/obo/GAZ_00260968 -->

    <owl:NamedIndividual rdf:about="http://purl.obolibrary.org/obo/GAZ_00260968">
        <obo:RO_0001025 rdf:resource="http://purl.obolibrary.org/obo/GAZ_00058782"/>
        <obo:IAO_0000115>A lake on the Luapula Floodplain.</obo:IAO_0000115>
        <oboInOwl:hasOBONamespace>GAZ</oboInOwl:hasOBONamespace>
        <oboInOwl:id>GAZ:00260968</oboInOwl:id>
        <rdfs:label>Lake Kainsa</rdfs:label>
    </owl:NamedIndividual>
    


    <!-- http://purl.obolibrary.org/obo/GAZ_00260969 -->

    <owl:NamedIndividual rdf:about="http://purl.obolibrary.org/obo/GAZ_00260969">
        <obo:RO_0001025 rdf:resource="http://purl.obolibrary.org/obo/GAZ_00058782"/>
        <obo:IAO_0000115>A lake on the Luapula Floodplain.</obo:IAO_0000115>
        <oboInOwl:hasOBONamespace>GAZ</oboInOwl:hasOBONamespace>
        <oboInOwl:id>GAZ:00260969</oboInOwl:id>
        <rdfs:label>Lake Kinseneka</rdfs:label>
    </owl:NamedIndividual>
    


    <!-- http://purl.obolibrary.org/obo/GAZ_00260970 -->

    <owl:NamedIndividual rdf:about="http://purl.obolibrary.org/obo/GAZ_00260970">
        <obo:RO_0001025 rdf:resource="http://purl.obolibrary.org/obo/GAZ_00041532"/>
        <obo:IAO_0000115>An island.</obo:IAO_0000115>
        <oboInOwl:hasOBONamespace>GAZ</oboInOwl:hasOBONamespace>
        <oboInOwl:id>GAZ:00260970</oboInOwl:id>
        <rdfs:label>Katima Island</rdfs:label>
    </owl:NamedIndividual>
    


    <!-- http://purl.obolibrary.org/obo/GAZ_00281373 -->

    <owl:NamedIndividual rdf:about="http://purl.obolibrary.org/obo/GAZ_00281373">
        <obo:RO_0001025 rdf:resource="http://purl.obolibrary.org/obo/GAZ_00123426"/>
        <obo:IAO_0000115>A populated place.</obo:IAO_0000115>
        <oboInOwl:hasOBONamespace>GAZ</oboInOwl:hasOBONamespace>
        <oboInOwl:id>GAZ:00281373</oboInOwl:id>
        <rdfs:label>Aramis</rdfs:label>
    </owl:NamedIndividual>
    


    <!-- http://purl.obolibrary.org/obo/GAZ_00281374 -->

    <owl:NamedIndividual rdf:about="http://purl.obolibrary.org/obo/GAZ_00281374">
        <obo:RO_0001025 rdf:resource="http://purl.obolibrary.org/obo/GAZ_00281373"/>
        <obo:IAO_0000115>A paleontogical site where remains of Australopithecus and Ardipithecus (Ardipithecus ramidus) have been found.</obo:IAO_0000115>
        <oboInOwl:hasOBONamespace>GAZ</oboInOwl:hasOBONamespace>
        <oboInOwl:id>GAZ:00281374</oboInOwl:id>
        <rdfs:label>Aramis [site]</rdfs:label>
    </owl:NamedIndividual>
    


    <!-- http://purl.obolibrary.org/obo/GAZ_00281375 -->

    <owl:NamedIndividual rdf:about="http://purl.obolibrary.org/obo/GAZ_00281375">
        <obo:RO_0001025 rdf:resource="http://purl.obolibrary.org/obo/GAZ_00123417"/>
        <obo:IAO_0000115>A paleontological site.</obo:IAO_0000115>
        <oboInOwl:hasOBONamespace>GAZ</oboInOwl:hasOBONamespace>
        <oboInOwl:id>GAZ:00281375</oboInOwl:id>
        <rdfs:label>Dikika</rdfs:label>
    </owl:NamedIndividual>
    


    <!-- http://purl.obolibrary.org/obo/GAZ_00281376 -->

    <owl:NamedIndividual rdf:about="http://purl.obolibrary.org/obo/GAZ_00281376">
        <obo:RO_0001025 rdf:resource="http://purl.obolibrary.org/obo/GAZ_00123417"/>
        <obo:IAO_0000115>A paleontogical site.</obo:IAO_0000115>
        <oboInOwl:hasOBONamespace>GAZ</oboInOwl:hasOBONamespace>
        <oboInOwl:id>GAZ:00281376</oboInOwl:id>
        <rdfs:label>Hadar [site]</rdfs:label>
    </owl:NamedIndividual>
    


    <!-- http://purl.obolibrary.org/obo/GAZ_00281377 -->

    <owl:NamedIndividual rdf:about="http://purl.obolibrary.org/obo/GAZ_00281377">
        <obo:RO_0001025 rdf:resource="http://purl.obolibrary.org/obo/GAZ_00000784"/>
        <obo:IAO_0000115>An archeological site. Palaeolithic. Located across the Awash River from the village of Melka Awash.</obo:IAO_0000115>
        <oboInOwl:hasOBONamespace>GAZ</oboInOwl:hasOBONamespace>
        <oboInOwl:id>GAZ:00281377</oboInOwl:id>
        <rdfs:label>Melka Kunture</rdfs:label>
    </owl:NamedIndividual>
    


    <!-- http://purl.obolibrary.org/obo/GAZ_00281432 -->

    <owl:NamedIndividual rdf:about="http://purl.obolibrary.org/obo/GAZ_00281432">
        <obo:RO_0001025 rdf:resource="http://purl.obolibrary.org/obo/GAZ_00124306"/>
        <obo:IAO_0000115>An archeological site. A Late Stone Age site in Mau Escarpment of Kenya.</obo:IAO_0000115>
        <oboInOwl:hasOBONamespace>GAZ</oboInOwl:hasOBONamespace>
        <oboInOwl:id>GAZ:00281432</oboInOwl:id>
        <rdfs:label>Enkapune Ya Muto</rdfs:label>
    </owl:NamedIndividual>
    


    <!-- http://purl.obolibrary.org/obo/GAZ_00281451 -->

    <owl:NamedIndividual rdf:about="http://purl.obolibrary.org/obo/GAZ_00281451">
        <obo:IAO_0000115>A single drop waterfall on the border of Zambia and Tanzania at the southeast end of Lake Tanganyika.</obo:IAO_0000115>
        <oboInOwl:hasOBONamespace>GAZ</oboInOwl:hasOBONamespace>
        <oboInOwl:id>GAZ:00281451</oboInOwl:id>
        <rdfs:label>Kalambo Falls</rdfs:label>
    </owl:NamedIndividual>
    


    <!-- 
    ///////////////////////////////////////////////////////////////////////////////////////
    //
    // Annotations
    //
    ///////////////////////////////////////////////////////////////////////////////////////
     -->

    <rdf:Description rdf:about="http://purl.obolibrary.org/obo/GAZ_00000778">
        <oboInOwl:hasOBONamespace>GAZ</oboInOwl:hasOBONamespace>
        <oboInOwl:id>GAZ:00000778</oboInOwl:id>
        <rdfs:label>Region (Ethiopia)</rdfs:label>
    </rdf:Description>
    <rdf:Description rdf:about="http://purl.obolibrary.org/obo/GAZ_00000779">
        <oboInOwl:id>GAZ:00000779</oboInOwl:id>
        <obo:IAO_0000115>One of the nine ethnic divisions (kililoch) of Ethiopia, and is the homeland of the Afar people. Formerly known as Region 2, its current capital is Asayita; a new capital named Semera on the paved Awash - Asseb highway is under construction.</obo:IAO_0000115>
        <rdfs:label>Afar Region</rdfs:label>
        <oboInOwl:hasOBONamespace>GAZ</oboInOwl:hasOBONamespace>
    </rdf:Description>
    <rdf:Description rdf:about="http://purl.obolibrary.org/obo/GAZ_00000780">
        <oboInOwl:hasOBONamespace>GAZ</oboInOwl:hasOBONamespace>
        <obo:IAO_0000115>One of the nine ethnic divisions (kililoch) of Ethiopia.</obo:IAO_0000115>
        <rdfs:label>Amhara Region</rdfs:label>
        <oboInOwl:id>GAZ:00000780</oboInOwl:id>
    </rdf:Description>
    <rdf:Description rdf:about="http://purl.obolibrary.org/obo/GAZ_00000781">
        <rdfs:label>Benishangul-Gumuz Region</rdfs:label>
        <oboInOwl:hasOBONamespace>GAZ</oboInOwl:hasOBONamespace>
        <obo:IAO_0000115>One of the nine ethnic divisions (kililoch) of Ethiopia. Region was created from the westernmost portion of the Gojjam province (the part north of the Abay River), and the northwestern portion of the Welega Province (the part south of the Abay).</obo:IAO_0000115>
        <oboInOwl:id>GAZ:00000781</oboInOwl:id>
    </rdf:Description>
    <rdf:Description rdf:about="http://purl.obolibrary.org/obo/GAZ_00000782">
        <rdfs:label>Gambela Peoples Region</rdfs:label>
        <oboInOwl:id>GAZ:00000782</oboInOwl:id>
        <oboInOwl:hasOBONamespace>GAZ</oboInOwl:hasOBONamespace>
        <obo:IAO_0000115>One of the nine ethnic divisions (kililoch) of Ethiopia. Its capital is Gambela. Lying between the Baro and Akobo Rivers, the western part of Gambela includes the Baro salient.</obo:IAO_0000115>
    </rdf:Description>
    <rdf:Description rdf:about="http://purl.obolibrary.org/obo/GAZ_00000783">
        <rdfs:label>Harari People Region</rdfs:label>
        <oboInOwl:id>GAZ:00000783</oboInOwl:id>
        <obo:IAO_0000115>One of the nine ethnic divisions (kililoch) of Ethiopia. An enclave in Oromia Region. It includes the former Arsi Province along with portions of the former Bale, Hararghe, Illubabor, Kaffa, Shewa, Sidamo, and Welega provinces. Its current capital is Adama.</obo:IAO_0000115>
        <oboInOwl:hasOBONamespace>GAZ</oboInOwl:hasOBONamespace>
    </rdf:Description>
    <rdf:Description rdf:about="http://purl.obolibrary.org/obo/GAZ_00000784">
        <rdfs:label>Oromia Region</rdfs:label>
        <oboInOwl:id>GAZ:00000784</oboInOwl:id>
        <oboInOwl:hasOBONamespace>GAZ</oboInOwl:hasOBONamespace>
        <obo:IAO_0000115>One of the nine ethnic divisions (kililoch) of Ethiopia.</obo:IAO_0000115>
    </rdf:Description>
    <rdf:Description rdf:about="http://purl.obolibrary.org/obo/GAZ_00000785">
        <obo:IAO_0000115>The eastern-most of the nine ethnic divisions (kililoch) of Ethiopia. The region borders Kenya to the south-west, the Ethopian regions of Oromia, Afar and Dire Dawa (Diridhawa) to the west, Djibouti to the north and Somalia to the north, east and south.</obo:IAO_0000115>
        <oboInOwl:id>GAZ:00000785</oboInOwl:id>
        <oboInOwl:hasOBONamespace>GAZ</oboInOwl:hasOBONamespace>
        <rdfs:label>Somali Region</rdfs:label>
    </rdf:Description>
    <rdf:Description rdf:about="http://purl.obolibrary.org/obo/GAZ_00000786">
        <obo:IAO_0000115>One of the nine ethnic divisions (kililoch) of Ethiopia. The SNNPR borders Kenya to the south, the Ilemi Triangle (a region claimed by Ethiopia, Kenya, and Sudan) to the southwest, Sudan to the west, the Ethiopian region of Gambela to the north, and the Ethiopian region of Oromia to the north and east. Besides Awasa, the region&apos;s major cities and towns include Arba Minch, Bonga, Chencha, Dila, Irgalem, Mizan Teferi, Sodo, Wendo, and Worabe.</obo:IAO_0000115>
        <oboInOwl:id>GAZ:00000786</oboInOwl:id>
        <rdfs:label>Southern Nations, Nationalities, and Peoples Region</rdfs:label>
        <oboInOwl:hasOBONamespace>GAZ</oboInOwl:hasOBONamespace>
    </rdf:Description>
    <rdf:Description rdf:about="http://purl.obolibrary.org/obo/GAZ_00000787">
        <rdfs:label>Tigray Region</rdfs:label>
        <obo:IAO_0000115>The northernmost of the nine ethnic regions (kililoch) of Ethiopia. Tigray is bordered by Eritrea to the north (independent from Ethiopia since 1993), Sudan to the west, the Afar Region to the east and the Amhara Region to the south. Besides Mek&apos;ele, other major towns and cities in Tigray include Abiy Addi, Adigrat, Adwa, Aksum, Humera (controversial), Inda Selassie, Korem, Alamata, Maychew, Wukro, Qwiha, and Zalambessa, as well as the historically significant village of Yeha.</obo:IAO_0000115>
        <oboInOwl:id>GAZ:00000787</oboInOwl:id>
        <oboInOwl:hasOBONamespace>GAZ</oboInOwl:hasOBONamespace>
    </rdf:Description>
    <rdf:Description rdf:about="http://purl.obolibrary.org/obo/GAZ_00001012">
        <oboInOwl:hasOBONamespace>GAZ</oboInOwl:hasOBONamespace>
        <rdfs:label>Administration (Ethiopia)</rdfs:label>
        <oboInOwl:id>GAZ:00001012</oboInOwl:id>
    </rdf:Description>
    <rdf:Description rdf:about="http://purl.obolibrary.org/obo/GAZ_00031091">
        <rdfs:label>Addis Ababa City</rdfs:label>
        <obo:IAO_0000115>The capital city of Ethiopia. As a chartered city (ras gez astedader), Addis Ababa has the status of both a city and a state.</obo:IAO_0000115>
        <oboInOwl:hasOBONamespace>GAZ</oboInOwl:hasOBONamespace>
        <oboInOwl:id>GAZ:00031091</oboInOwl:id>
    </rdf:Description>
    <rdf:Description rdf:about="http://purl.obolibrary.org/obo/GAZ_00031092">
        <oboInOwl:id>GAZ:00031092</oboInOwl:id>
        <rdfs:label>Dire Dawa City</rdfs:label>
        <obo:IAO_0000115>One of two chartered cities (astedader akabibi) in Ethiopia.</obo:IAO_0000115>
        <oboInOwl:hasOBONamespace>GAZ</oboInOwl:hasOBONamespace>
    </rdf:Description>
</rdf:RDF>



<!-- Generated by the OWL API (version 4.5.6) https://github.com/owlcs/owlapi -->

