<?xml version="1.0"?>
<rdf:RDF xmlns="http://purl.obolibrary.org/obo/gaz/subsets/countries/Gabon.owl#"
     xml:base="http://purl.obolibrary.org/obo/gaz/subsets/countries/Gabon.owl"
     xmlns:obo="http://purl.obolibrary.org/obo/"
     xmlns:owl="http://www.w3.org/2002/07/owl#"
     xmlns:rdf="http://www.w3.org/1999/02/22-rdf-syntax-ns#"
     xmlns:xml="http://www.w3.org/XML/1998/namespace"
     xmlns:xsd="http://www.w3.org/2001/XMLSchema#"
     xmlns:rdfs="http://www.w3.org/2000/01/rdf-schema#"
     xmlns:oboInOwl="http://www.geneontology.org/formats/oboInOwl#">
    <owl:Ontology rdf:about="http://purl.obolibrary.org/obo/gaz/subsets/countries/Gabon.owl">
        <owl:imports rdf:resource="http://purl.obolibrary.org/obo/gaz/imports/envo_import.owl"/>
        <owl:imports rdf:resource="http://purl.obolibrary.org/obo/gaz/imports/ro_import.owl"/>
    </owl:Ontology>
    


    <!-- 
    ///////////////////////////////////////////////////////////////////////////////////////
    //
    // Annotation properties
    //
    ///////////////////////////////////////////////////////////////////////////////////////
     -->

    


    <!-- http://purl.obolibrary.org/obo/IAO_0000115 -->

    <owl:AnnotationProperty rdf:about="http://purl.obolibrary.org/obo/IAO_0000115"/>
    


    <!-- http://www.geneontology.org/formats/oboInOwl#hasOBONamespace -->

    <owl:AnnotationProperty rdf:about="http://www.geneontology.org/formats/oboInOwl#hasOBONamespace"/>
    


    <!-- http://www.geneontology.org/formats/oboInOwl#id -->

    <owl:AnnotationProperty rdf:about="http://www.geneontology.org/formats/oboInOwl#id"/>
    


    <!-- 
    ///////////////////////////////////////////////////////////////////////////////////////
    //
    // Object Properties
    //
    ///////////////////////////////////////////////////////////////////////////////////////
     -->

    


    <!-- http://purl.obolibrary.org/obo/RO_0001025 -->

    <owl:ObjectProperty rdf:about="http://purl.obolibrary.org/obo/RO_0001025"/>
    


    <!-- 
    ///////////////////////////////////////////////////////////////////////////////////////
    //
    // Classes
    //
    ///////////////////////////////////////////////////////////////////////////////////////
     -->

    


    <!-- http://purl.obolibrary.org/obo/ENVO_00000009 -->

    <owl:Class rdf:about="http://purl.obolibrary.org/obo/ENVO_00000009"/>
    


    <!-- http://purl.obolibrary.org/obo/ENVO_00000856 -->

    <owl:Class rdf:about="http://purl.obolibrary.org/obo/ENVO_00000856"/>
    


    <!-- http://purl.obolibrary.org/obo/GAZ_00005666 -->

    <owl:Class rdf:about="http://purl.obolibrary.org/obo/GAZ_00005666"/>
    


    <!-- http://purl.obolibrary.org/obo/GAZ_00005667 -->

    <owl:Class rdf:about="http://purl.obolibrary.org/obo/GAZ_00005667">
        <rdfs:subClassOf rdf:resource="http://purl.obolibrary.org/obo/GAZ_00005666"/>
    </owl:Class>
    


    <!-- http://purl.obolibrary.org/obo/GAZ_00005668 -->

    <owl:Class rdf:about="http://purl.obolibrary.org/obo/GAZ_00005668">
        <rdfs:subClassOf rdf:resource="http://purl.obolibrary.org/obo/GAZ_00005669"/>
    </owl:Class>
    


    <!-- http://purl.obolibrary.org/obo/GAZ_00005669 -->

    <owl:Class rdf:about="http://purl.obolibrary.org/obo/GAZ_00005669"/>
    


    <!-- http://purl.obolibrary.org/obo/GAZ_00005670 -->

    <owl:Class rdf:about="http://purl.obolibrary.org/obo/GAZ_00005670">
        <rdfs:subClassOf rdf:resource="http://purl.obolibrary.org/obo/GAZ_00005666"/>
    </owl:Class>
    


    <!-- http://purl.obolibrary.org/obo/GAZ_00005671 -->

    <owl:Class rdf:about="http://purl.obolibrary.org/obo/GAZ_00005671">
        <rdfs:subClassOf rdf:resource="http://purl.obolibrary.org/obo/GAZ_00005669"/>
    </owl:Class>
    


    <!-- http://purl.obolibrary.org/obo/GAZ_00005672 -->

    <owl:Class rdf:about="http://purl.obolibrary.org/obo/GAZ_00005672">
        <rdfs:subClassOf rdf:resource="http://purl.obolibrary.org/obo/GAZ_00005666"/>
    </owl:Class>
    


    <!-- http://purl.obolibrary.org/obo/GAZ_00005673 -->

    <owl:Class rdf:about="http://purl.obolibrary.org/obo/GAZ_00005673">
        <rdfs:subClassOf rdf:resource="http://purl.obolibrary.org/obo/GAZ_00005669"/>
    </owl:Class>
    


    <!-- http://purl.obolibrary.org/obo/GAZ_00008121 -->

    <owl:Class rdf:about="http://purl.obolibrary.org/obo/GAZ_00008121">
        <rdfs:subClassOf rdf:resource="http://purl.obolibrary.org/obo/GAZ_00005666"/>
    </owl:Class>
    


    <!-- http://purl.obolibrary.org/obo/GAZ_00008122 -->

    <owl:Class rdf:about="http://purl.obolibrary.org/obo/GAZ_00008122">
        <rdfs:subClassOf rdf:resource="http://purl.obolibrary.org/obo/GAZ_00005666"/>
    </owl:Class>
    


    <!-- http://purl.obolibrary.org/obo/GAZ_00008123 -->

    <owl:Class rdf:about="http://purl.obolibrary.org/obo/GAZ_00008123">
        <rdfs:subClassOf rdf:resource="http://purl.obolibrary.org/obo/GAZ_00005666"/>
    </owl:Class>
    


    <!-- http://purl.obolibrary.org/obo/GAZ_00008124 -->

    <owl:Class rdf:about="http://purl.obolibrary.org/obo/GAZ_00008124">
        <rdfs:subClassOf rdf:resource="http://purl.obolibrary.org/obo/GAZ_00005666"/>
    </owl:Class>
    


    <!-- http://purl.obolibrary.org/obo/GAZ_00008125 -->

    <owl:Class rdf:about="http://purl.obolibrary.org/obo/GAZ_00008125">
        <rdfs:subClassOf rdf:resource="http://purl.obolibrary.org/obo/GAZ_00005666"/>
    </owl:Class>
    


    <!-- http://purl.obolibrary.org/obo/GAZ_00008126 -->

    <owl:Class rdf:about="http://purl.obolibrary.org/obo/GAZ_00008126">
        <rdfs:subClassOf rdf:resource="http://purl.obolibrary.org/obo/GAZ_00005666"/>
    </owl:Class>
    


    <!-- http://purl.obolibrary.org/obo/GAZ_00008127 -->

    <owl:Class rdf:about="http://purl.obolibrary.org/obo/GAZ_00008127">
        <rdfs:subClassOf rdf:resource="http://purl.obolibrary.org/obo/GAZ_00005669"/>
    </owl:Class>
    


    <!-- http://purl.obolibrary.org/obo/GAZ_00009929 -->

    <owl:Class rdf:about="http://purl.obolibrary.org/obo/GAZ_00009929">
        <rdfs:subClassOf rdf:resource="http://purl.obolibrary.org/obo/GAZ_00005669"/>
    </owl:Class>
    


    <!-- http://purl.obolibrary.org/obo/GAZ_00009930 -->

    <owl:Class rdf:about="http://purl.obolibrary.org/obo/GAZ_00009930">
        <rdfs:subClassOf rdf:resource="http://purl.obolibrary.org/obo/GAZ_00005669"/>
    </owl:Class>
    


    <!-- http://purl.obolibrary.org/obo/GAZ_00009931 -->

    <owl:Class rdf:about="http://purl.obolibrary.org/obo/GAZ_00009931">
        <rdfs:subClassOf rdf:resource="http://purl.obolibrary.org/obo/GAZ_00005669"/>
    </owl:Class>
    


    <!-- http://purl.obolibrary.org/obo/GAZ_00009934 -->

    <owl:Class rdf:about="http://purl.obolibrary.org/obo/GAZ_00009934">
        <rdfs:subClassOf rdf:resource="http://purl.obolibrary.org/obo/GAZ_00005669"/>
    </owl:Class>
    


    <!-- http://purl.obolibrary.org/obo/GAZ_00052686 -->

    <owl:Class rdf:about="http://purl.obolibrary.org/obo/GAZ_00052686">
        <rdfs:subClassOf rdf:resource="http://purl.obolibrary.org/obo/GAZ_00005669"/>
    </owl:Class>
    


    <!-- http://purl.obolibrary.org/obo/GAZ_00052688 -->

    <owl:Class rdf:about="http://purl.obolibrary.org/obo/GAZ_00052688">
        <rdfs:subClassOf rdf:resource="http://purl.obolibrary.org/obo/GAZ_00005669"/>
    </owl:Class>
    


    <!-- http://purl.obolibrary.org/obo/GAZ_00052690 -->

    <owl:Class rdf:about="http://purl.obolibrary.org/obo/GAZ_00052690">
        <rdfs:subClassOf rdf:resource="http://purl.obolibrary.org/obo/GAZ_00005669"/>
    </owl:Class>
    


    <!-- http://purl.obolibrary.org/obo/GAZ_00052694 -->

    <owl:Class rdf:about="http://purl.obolibrary.org/obo/GAZ_00052694">
        <rdfs:subClassOf rdf:resource="http://purl.obolibrary.org/obo/GAZ_00005669"/>
    </owl:Class>
    


    <!-- http://purl.obolibrary.org/obo/GAZ_00052696 -->

    <owl:Class rdf:about="http://purl.obolibrary.org/obo/GAZ_00052696">
        <rdfs:subClassOf rdf:resource="http://purl.obolibrary.org/obo/GAZ_00005669"/>
    </owl:Class>
    


    <!-- http://purl.obolibrary.org/obo/GAZ_00052699 -->

    <owl:Class rdf:about="http://purl.obolibrary.org/obo/GAZ_00052699">
        <rdfs:subClassOf rdf:resource="http://purl.obolibrary.org/obo/GAZ_00005669"/>
    </owl:Class>
    


    <!-- http://purl.obolibrary.org/obo/GAZ_00052701 -->

    <owl:Class rdf:about="http://purl.obolibrary.org/obo/GAZ_00052701">
        <rdfs:subClassOf rdf:resource="http://purl.obolibrary.org/obo/GAZ_00005669"/>
    </owl:Class>
    


    <!-- http://purl.obolibrary.org/obo/GAZ_00052702 -->

    <owl:Class rdf:about="http://purl.obolibrary.org/obo/GAZ_00052702">
        <rdfs:subClassOf rdf:resource="http://purl.obolibrary.org/obo/GAZ_00005669"/>
        <obo:IAO_0000115>A populated place. in N Gabon on the Ivindo River.</obo:IAO_0000115>
        <oboInOwl:hasOBONamespace>GAZ</oboInOwl:hasOBONamespace>
        <oboInOwl:id>GAZ:00052702</oboInOwl:id>
        <rdfs:label>Mayibout</rdfs:label>
    </owl:Class>
    


    <!-- http://purl.obolibrary.org/obo/GAZ_00052705 -->

    <owl:Class rdf:about="http://purl.obolibrary.org/obo/GAZ_00052705">
        <rdfs:subClassOf rdf:resource="http://purl.obolibrary.org/obo/GAZ_00005669"/>
    </owl:Class>
    


    <!-- http://purl.obolibrary.org/obo/GAZ_00052706 -->

    <owl:Class rdf:about="http://purl.obolibrary.org/obo/GAZ_00052706">
        <rdfs:subClassOf rdf:resource="http://purl.obolibrary.org/obo/GAZ_00005669"/>
    </owl:Class>
    


    <!-- http://purl.obolibrary.org/obo/GAZ_00052709 -->

    <owl:Class rdf:about="http://purl.obolibrary.org/obo/GAZ_00052709">
        <rdfs:subClassOf rdf:resource="http://purl.obolibrary.org/obo/GAZ_00005669"/>
    </owl:Class>
    


    <!-- http://purl.obolibrary.org/obo/GAZ_00052715 -->

    <owl:Class rdf:about="http://purl.obolibrary.org/obo/GAZ_00052715">
        <rdfs:subClassOf rdf:resource="http://purl.obolibrary.org/obo/GAZ_00005669"/>
    </owl:Class>
    


    <!-- http://purl.obolibrary.org/obo/GAZ_00052719 -->

    <owl:Class rdf:about="http://purl.obolibrary.org/obo/GAZ_00052719">
        <rdfs:subClassOf rdf:resource="http://purl.obolibrary.org/obo/GAZ_00005669"/>
    </owl:Class>
    


    <!-- http://purl.obolibrary.org/obo/GAZ_00052724 -->

    <owl:Class rdf:about="http://purl.obolibrary.org/obo/GAZ_00052724">
        <rdfs:subClassOf rdf:resource="http://purl.obolibrary.org/obo/GAZ_00005669"/>
    </owl:Class>
    


    <!-- http://purl.obolibrary.org/obo/GAZ_00052725 -->

    <owl:Class rdf:about="http://purl.obolibrary.org/obo/GAZ_00052725">
        <rdfs:subClassOf rdf:resource="http://purl.obolibrary.org/obo/GAZ_00005669"/>
    </owl:Class>
    


    <!-- http://purl.obolibrary.org/obo/GAZ_00052729 -->

    <owl:Class rdf:about="http://purl.obolibrary.org/obo/GAZ_00052729">
        <rdfs:subClassOf rdf:resource="http://purl.obolibrary.org/obo/GAZ_00005669"/>
    </owl:Class>
    


    <!-- http://purl.obolibrary.org/obo/GAZ_00052730 -->

    <owl:Class rdf:about="http://purl.obolibrary.org/obo/GAZ_00052730">
        <rdfs:subClassOf rdf:resource="http://purl.obolibrary.org/obo/GAZ_00005669"/>
    </owl:Class>
    


    <!-- http://purl.obolibrary.org/obo/GAZ_00052731 -->

    <owl:Class rdf:about="http://purl.obolibrary.org/obo/GAZ_00052731">
        <rdfs:subClassOf rdf:resource="http://purl.obolibrary.org/obo/GAZ_00005669"/>
    </owl:Class>
    


    <!-- http://purl.obolibrary.org/obo/GAZ_22223534 -->

    <owl:Class rdf:about="http://purl.obolibrary.org/obo/GAZ_22223534">
        <rdfs:subClassOf rdf:resource="http://purl.obolibrary.org/obo/GAZ_00005669"/>
    </owl:Class>
    


    <!-- 
    ///////////////////////////////////////////////////////////////////////////////////////
    //
    // Individuals
    //
    ///////////////////////////////////////////////////////////////////////////////////////
     -->

    


    <!-- http://purl.obolibrary.org/obo/GAZ_00001092 -->

    <owl:NamedIndividual rdf:about="http://purl.obolibrary.org/obo/GAZ_00001092">
        <rdf:type rdf:resource="http://purl.obolibrary.org/obo/ENVO_00000009"/>
        <obo:IAO_0000115>A country in west central Africa sharing borders with Equatorial Guinea, Cameroon, Republic of the Congo and the Gulf of Guinea. The capital and largest city is Libreville. Gabon is divided into 9 provinces and further divided into 37 departments.</obo:IAO_0000115>
        <oboInOwl:hasOBONamespace>GAZ</oboInOwl:hasOBONamespace>
        <oboInOwl:id>GAZ:00001092</oboInOwl:id>
        <rdfs:label>Gabon</rdfs:label>
    </owl:NamedIndividual>
    


    <!-- http://purl.obolibrary.org/obo/GAZ_00005666 -->

    <owl:NamedIndividual rdf:about="http://purl.obolibrary.org/obo/GAZ_00005666">
        <obo:RO_0001025 rdf:resource="http://purl.obolibrary.org/obo/GAZ_00001092"/>
    </owl:NamedIndividual>
    


    <!-- http://purl.obolibrary.org/obo/GAZ_00005667 -->

    <owl:NamedIndividual rdf:about="http://purl.obolibrary.org/obo/GAZ_00005667"/>
    


    <!-- http://purl.obolibrary.org/obo/GAZ_00005668 -->

    <owl:NamedIndividual rdf:about="http://purl.obolibrary.org/obo/GAZ_00005668">
        <rdf:type rdf:resource="http://purl.obolibrary.org/obo/ENVO_00000856"/>
        <obo:RO_0001025 rdf:resource="http://purl.obolibrary.org/obo/GAZ_02000554"/>
    </owl:NamedIndividual>
    


    <!-- http://purl.obolibrary.org/obo/GAZ_00005669 -->

    <owl:NamedIndividual rdf:about="http://purl.obolibrary.org/obo/GAZ_00005669">
        <obo:RO_0001025 rdf:resource="http://purl.obolibrary.org/obo/GAZ_00001092"/>
    </owl:NamedIndividual>
    


    <!-- http://purl.obolibrary.org/obo/GAZ_00005670 -->

    <owl:NamedIndividual rdf:about="http://purl.obolibrary.org/obo/GAZ_00005670"/>
    


    <!-- http://purl.obolibrary.org/obo/GAZ_00005671 -->

    <owl:NamedIndividual rdf:about="http://purl.obolibrary.org/obo/GAZ_00005671">
        <obo:RO_0001025 rdf:resource="http://purl.obolibrary.org/obo/GAZ_00005670"/>
    </owl:NamedIndividual>
    


    <!-- http://purl.obolibrary.org/obo/GAZ_00005672 -->

    <owl:NamedIndividual rdf:about="http://purl.obolibrary.org/obo/GAZ_00005672"/>
    


    <!-- http://purl.obolibrary.org/obo/GAZ_00005673 -->

    <owl:NamedIndividual rdf:about="http://purl.obolibrary.org/obo/GAZ_00005673">
        <obo:RO_0001025 rdf:resource="http://purl.obolibrary.org/obo/GAZ_00009933"/>
    </owl:NamedIndividual>
    


    <!-- http://purl.obolibrary.org/obo/GAZ_00005674 -->

    <owl:NamedIndividual rdf:about="http://purl.obolibrary.org/obo/GAZ_00005674">
        <obo:RO_0001025 rdf:resource="http://purl.obolibrary.org/obo/GAZ_00005671"/>
        <obo:IAO_0000115>A port city in Gabon, forming a south western suburb of Libreville.</obo:IAO_0000115>
        <oboInOwl:hasOBONamespace>GAZ</oboInOwl:hasOBONamespace>
        <oboInOwl:id>GAZ:00005674</oboInOwl:id>
        <rdfs:label>Owendo</rdfs:label>
    </owl:NamedIndividual>
    


    <!-- http://purl.obolibrary.org/obo/GAZ_00005675 -->

    <owl:NamedIndividual rdf:about="http://purl.obolibrary.org/obo/GAZ_00005675">
        <obo:RO_0001025 rdf:resource="http://purl.obolibrary.org/obo/GAZ_00005671"/>
        <oboInOwl:hasOBONamespace>GAZ</oboInOwl:hasOBONamespace>
        <oboInOwl:id>GAZ:00005675</oboInOwl:id>
        <rdfs:label>Foret de La Mondah</rdfs:label>
    </owl:NamedIndividual>
    


    <!-- http://purl.obolibrary.org/obo/GAZ_00005678 -->

    <owl:NamedIndividual rdf:about="http://purl.obolibrary.org/obo/GAZ_00005678">
        <obo:RO_0001025 rdf:resource="http://purl.obolibrary.org/obo/GAZ_00235675"/>
        <oboInOwl:hasOBONamespace>GAZ</oboInOwl:hasOBONamespace>
        <oboInOwl:id>GAZ:00005678</oboInOwl:id>
        <rdfs:label>Ile aux Chauves-Souris</rdfs:label>
    </owl:NamedIndividual>
    


    <!-- http://purl.obolibrary.org/obo/GAZ_00008121 -->

    <owl:NamedIndividual rdf:about="http://purl.obolibrary.org/obo/GAZ_00008121"/>
    


    <!-- http://purl.obolibrary.org/obo/GAZ_00008122 -->

    <owl:NamedIndividual rdf:about="http://purl.obolibrary.org/obo/GAZ_00008122"/>
    


    <!-- http://purl.obolibrary.org/obo/GAZ_00008123 -->

    <owl:NamedIndividual rdf:about="http://purl.obolibrary.org/obo/GAZ_00008123"/>
    


    <!-- http://purl.obolibrary.org/obo/GAZ_00008124 -->

    <owl:NamedIndividual rdf:about="http://purl.obolibrary.org/obo/GAZ_00008124"/>
    


    <!-- http://purl.obolibrary.org/obo/GAZ_00008125 -->

    <owl:NamedIndividual rdf:about="http://purl.obolibrary.org/obo/GAZ_00008125"/>
    


    <!-- http://purl.obolibrary.org/obo/GAZ_00008126 -->

    <owl:NamedIndividual rdf:about="http://purl.obolibrary.org/obo/GAZ_00008126"/>
    


    <!-- http://purl.obolibrary.org/obo/GAZ_00008127 -->

    <owl:NamedIndividual rdf:about="http://purl.obolibrary.org/obo/GAZ_00008127">
        <obo:RO_0001025 rdf:resource="http://purl.obolibrary.org/obo/GAZ_02000561"/>
    </owl:NamedIndividual>
    


    <!-- http://purl.obolibrary.org/obo/GAZ_00009927 -->

    <owl:NamedIndividual rdf:about="http://purl.obolibrary.org/obo/GAZ_00009927">
        <obo:RO_0001025 rdf:resource="http://purl.obolibrary.org/obo/GAZ_00005672"/>
        <obo:IAO_0000115>A department of Ogooue-Ivindo Province in northern-eastern Gabon. The capital lies at Mekambo.</obo:IAO_0000115>
        <oboInOwl:hasOBONamespace>GAZ</oboInOwl:hasOBONamespace>
        <oboInOwl:id>GAZ:00009927</oboInOwl:id>
        <rdfs:label>Zadie Department</rdfs:label>
    </owl:NamedIndividual>
    


    <!-- http://purl.obolibrary.org/obo/GAZ_00009929 -->

    <owl:NamedIndividual rdf:about="http://purl.obolibrary.org/obo/GAZ_00009929">
        <obo:RO_0001025 rdf:resource="http://purl.obolibrary.org/obo/GAZ_00005672"/>
    </owl:NamedIndividual>
    


    <!-- http://purl.obolibrary.org/obo/GAZ_00009930 -->

    <owl:NamedIndividual rdf:about="http://purl.obolibrary.org/obo/GAZ_00009930">
        <rdf:type rdf:resource="http://purl.obolibrary.org/obo/ENVO_00000856"/>
        <obo:RO_0001025 rdf:resource="http://purl.obolibrary.org/obo/GAZ_02000559"/>
    </owl:NamedIndividual>
    


    <!-- http://purl.obolibrary.org/obo/GAZ_00009931 -->

    <owl:NamedIndividual rdf:about="http://purl.obolibrary.org/obo/GAZ_00009931">
        <rdf:type rdf:resource="http://purl.obolibrary.org/obo/ENVO_00000856"/>
        <obo:RO_0001025 rdf:resource="http://purl.obolibrary.org/obo/GAZ_00009927"/>
    </owl:NamedIndividual>
    


    <!-- http://purl.obolibrary.org/obo/GAZ_00009932 -->

    <owl:NamedIndividual rdf:about="http://purl.obolibrary.org/obo/GAZ_00009932">
        <obo:RO_0001025 rdf:resource="http://purl.obolibrary.org/obo/GAZ_00009931"/>
        <oboInOwl:hasOBONamespace>GAZ</oboInOwl:hasOBONamespace>
        <oboInOwl:id>GAZ:00009932</oboInOwl:id>
        <rdfs:label>Grand-Etoumbi</rdfs:label>
    </owl:NamedIndividual>
    


    <!-- http://purl.obolibrary.org/obo/GAZ_00009933 -->

    <owl:NamedIndividual rdf:about="http://purl.obolibrary.org/obo/GAZ_00009933">
        <obo:RO_0001025 rdf:resource="http://purl.obolibrary.org/obo/GAZ_00005672"/>
        <obo:IAO_0000115>A department of Ogooue-Ivindo Province in northern-central Gabon. The capital lies at Makokou.</obo:IAO_0000115>
        <oboInOwl:hasOBONamespace>GAZ</oboInOwl:hasOBONamespace>
        <oboInOwl:id>GAZ:00009933</oboInOwl:id>
        <rdfs:label>Ivindo Department</rdfs:label>
    </owl:NamedIndividual>
    


    <!-- http://purl.obolibrary.org/obo/GAZ_00009934 -->

    <owl:NamedIndividual rdf:about="http://purl.obolibrary.org/obo/GAZ_00009934">
        <obo:RO_0001025 rdf:resource="http://purl.obolibrary.org/obo/GAZ_00005672"/>
    </owl:NamedIndividual>
    


    <!-- http://purl.obolibrary.org/obo/GAZ_00009935 -->

    <owl:NamedIndividual rdf:about="http://purl.obolibrary.org/obo/GAZ_00009935">
        <obo:RO_0001025 rdf:resource="http://purl.obolibrary.org/obo/GAZ_00009934"/>
        <oboInOwl:hasOBONamespace>GAZ</oboInOwl:hasOBONamespace>
        <oboInOwl:id>GAZ:00009935</oboInOwl:id>
        <rdfs:label>Olloba</rdfs:label>
    </owl:NamedIndividual>
    


    <!-- http://purl.obolibrary.org/obo/GAZ_00031329 -->

    <owl:NamedIndividual rdf:about="http://purl.obolibrary.org/obo/GAZ_00031329">
        <obo:RO_0001025 rdf:resource="http://purl.obolibrary.org/obo/GAZ_00008126"/>
        <obo:IAO_0000115>A department of Woleu-Ntem Province in northern Gabon. The capital lies at Mitzic.</obo:IAO_0000115>
        <oboInOwl:hasOBONamespace>GAZ</oboInOwl:hasOBONamespace>
        <oboInOwl:id>GAZ:00031329</oboInOwl:id>
        <rdfs:label>Okano Department</rdfs:label>
    </owl:NamedIndividual>
    


    <!-- http://purl.obolibrary.org/obo/GAZ_00031330 -->

    <owl:NamedIndividual rdf:about="http://purl.obolibrary.org/obo/GAZ_00031330">
        <obo:RO_0001025 rdf:resource="http://purl.obolibrary.org/obo/GAZ_00008126"/>
        <obo:IAO_0000115>A department of Woleu-Ntem Province in northern Gabon. The capital lies at Medouneu.</obo:IAO_0000115>
        <oboInOwl:hasOBONamespace>GAZ</oboInOwl:hasOBONamespace>
        <oboInOwl:id>GAZ:00031330</oboInOwl:id>
        <rdfs:label>Haut-Ntem Department</rdfs:label>
    </owl:NamedIndividual>
    


    <!-- http://purl.obolibrary.org/obo/GAZ_00031331 -->

    <owl:NamedIndividual rdf:about="http://purl.obolibrary.org/obo/GAZ_00031331">
        <obo:RO_0001025 rdf:resource="http://purl.obolibrary.org/obo/GAZ_00008126"/>
        <obo:IAO_0000115>A department of Woleu-Ntem Province in northern Gabon. The capital lies at Ndindi. The department borders with Equatorial Guinea.</obo:IAO_0000115>
        <oboInOwl:hasOBONamespace>GAZ</oboInOwl:hasOBONamespace>
        <oboInOwl:id>GAZ:00031331</oboInOwl:id>
        <rdfs:label>Haut-Komo Department</rdfs:label>
    </owl:NamedIndividual>
    


    <!-- http://purl.obolibrary.org/obo/GAZ_00031332 -->

    <owl:NamedIndividual rdf:about="http://purl.obolibrary.org/obo/GAZ_00031332">
        <obo:RO_0001025 rdf:resource="http://purl.obolibrary.org/obo/GAZ_00008126"/>
        <obo:IAO_0000115>A department of Woleu-Ntem Province in northern Gabon. The capital lies at Bitam. It borders Equatorial Guinea and Cameroon.</obo:IAO_0000115>
        <oboInOwl:hasOBONamespace>GAZ</oboInOwl:hasOBONamespace>
        <oboInOwl:id>GAZ:00031332</oboInOwl:id>
        <rdfs:label>Ntem Department</rdfs:label>
    </owl:NamedIndividual>
    


    <!-- http://purl.obolibrary.org/obo/GAZ_00031333 -->

    <owl:NamedIndividual rdf:about="http://purl.obolibrary.org/obo/GAZ_00031333">
        <obo:RO_0001025 rdf:resource="http://purl.obolibrary.org/obo/GAZ_00008126"/>
        <obo:IAO_0000115>A department of Woleu-Ntem Province in northern Gabon. The capital lies at Oyem. It borders Equatorial Guinea to the west.</obo:IAO_0000115>
        <oboInOwl:hasOBONamespace>GAZ</oboInOwl:hasOBONamespace>
        <oboInOwl:id>GAZ:00031333</oboInOwl:id>
        <rdfs:label>Woleu Department</rdfs:label>
    </owl:NamedIndividual>
    


    <!-- http://purl.obolibrary.org/obo/GAZ_00031334 -->

    <owl:NamedIndividual rdf:about="http://purl.obolibrary.org/obo/GAZ_00031334">
        <obo:RO_0001025 rdf:resource="http://purl.obolibrary.org/obo/GAZ_00008125"/>
        <obo:IAO_0000115>A department of Ogooue-Lolo Province in eastern Gabon. The capital lies at Pana.</obo:IAO_0000115>
        <oboInOwl:hasOBONamespace>GAZ</oboInOwl:hasOBONamespace>
        <oboInOwl:id>GAZ:00031334</oboInOwl:id>
        <rdfs:label>Lombo-Bouenguidi Department</rdfs:label>
    </owl:NamedIndividual>
    


    <!-- http://purl.obolibrary.org/obo/GAZ_00031335 -->

    <owl:NamedIndividual rdf:about="http://purl.obolibrary.org/obo/GAZ_00031335">
        <obo:RO_0001025 rdf:resource="http://purl.obolibrary.org/obo/GAZ_00008125"/>
        <obo:IAO_0000115>A department of Ogooue-Lolo Province in eastern Gabon. The capital lies at Lastoursville.</obo:IAO_0000115>
        <oboInOwl:hasOBONamespace>GAZ</oboInOwl:hasOBONamespace>
        <oboInOwl:id>GAZ:00031335</oboInOwl:id>
        <rdfs:label>Mouloundou Department</rdfs:label>
    </owl:NamedIndividual>
    


    <!-- http://purl.obolibrary.org/obo/GAZ_00031336 -->

    <owl:NamedIndividual rdf:about="http://purl.obolibrary.org/obo/GAZ_00031336">
        <obo:RO_0001025 rdf:resource="http://purl.obolibrary.org/obo/GAZ_00008125"/>
        <obo:IAO_0000115>A department of Ogooue-Lolo Province in central-eastern Gabon. The capital lies at Koulamoutou.</obo:IAO_0000115>
        <oboInOwl:hasOBONamespace>GAZ</oboInOwl:hasOBONamespace>
        <oboInOwl:id>GAZ:00031336</oboInOwl:id>
        <rdfs:label>Lolo-Bouenguidi Department</rdfs:label>
    </owl:NamedIndividual>
    


    <!-- http://purl.obolibrary.org/obo/GAZ_00031337 -->

    <owl:NamedIndividual rdf:about="http://purl.obolibrary.org/obo/GAZ_00031337">
        <obo:RO_0001025 rdf:resource="http://purl.obolibrary.org/obo/GAZ_00005672"/>
        <obo:IAO_0000115>A department of Ogooue-Ivindo Province in northern-centralGabon. The capital lies at Ovan.</obo:IAO_0000115>
        <oboInOwl:hasOBONamespace>GAZ</oboInOwl:hasOBONamespace>
        <oboInOwl:id>GAZ:00031337</oboInOwl:id>
        <rdfs:label>Mvoung Department</rdfs:label>
    </owl:NamedIndividual>
    


    <!-- http://purl.obolibrary.org/obo/GAZ_00031338 -->

    <owl:NamedIndividual rdf:about="http://purl.obolibrary.org/obo/GAZ_00031338">
        <obo:RO_0001025 rdf:resource="http://purl.obolibrary.org/obo/GAZ_00008124"/>
        <obo:IAO_0000115>A department of Nyanga Province in south-western Gabon. It is the most southernly department in Gabon and borders the Republic of the Congo. The capital lies at Minvoul.</obo:IAO_0000115>
        <oboInOwl:hasOBONamespace>GAZ</oboInOwl:hasOBONamespace>
        <oboInOwl:id>GAZ:00031338</oboInOwl:id>
        <rdfs:label>Haute-Banio Department</rdfs:label>
    </owl:NamedIndividual>
    


    <!-- http://purl.obolibrary.org/obo/GAZ_00031339 -->

    <owl:NamedIndividual rdf:about="http://purl.obolibrary.org/obo/GAZ_00031339">
        <obo:RO_0001025 rdf:resource="http://purl.obolibrary.org/obo/GAZ_00008124"/>
        <obo:IAO_0000115>A department of Nyanga Province in southern Gabon. The capital lies at Tchibanga.</obo:IAO_0000115>
        <oboInOwl:hasOBONamespace>GAZ</oboInOwl:hasOBONamespace>
        <oboInOwl:id>GAZ:00031339</oboInOwl:id>
        <rdfs:label>Mougoutsi Department</rdfs:label>
    </owl:NamedIndividual>
    


    <!-- http://purl.obolibrary.org/obo/GAZ_00031340 -->

    <owl:NamedIndividual rdf:about="http://purl.obolibrary.org/obo/GAZ_00031340">
        <obo:RO_0001025 rdf:resource="http://purl.obolibrary.org/obo/GAZ_00008124"/>
        <obo:IAO_0000115>A department of Nyanga Province in southern Gabon. The capital lies at Mayumba.</obo:IAO_0000115>
        <oboInOwl:hasOBONamespace>GAZ</oboInOwl:hasOBONamespace>
        <oboInOwl:id>GAZ:00031340</oboInOwl:id>
        <rdfs:label>Basse-Banio Department</rdfs:label>
    </owl:NamedIndividual>
    


    <!-- http://purl.obolibrary.org/obo/GAZ_00031341 -->

    <owl:NamedIndividual rdf:about="http://purl.obolibrary.org/obo/GAZ_00031341">
        <obo:RO_0001025 rdf:resource="http://purl.obolibrary.org/obo/GAZ_00008124"/>
        <obo:IAO_0000115>A department of Nyanga Province in southern Gabon. The capital lies at Moabi.</obo:IAO_0000115>
        <oboInOwl:hasOBONamespace>GAZ</oboInOwl:hasOBONamespace>
        <oboInOwl:id>GAZ:00031341</oboInOwl:id>
        <rdfs:label>Douigni Department</rdfs:label>
    </owl:NamedIndividual>
    


    <!-- http://purl.obolibrary.org/obo/GAZ_00031342 -->

    <owl:NamedIndividual rdf:about="http://purl.obolibrary.org/obo/GAZ_00031342">
        <obo:RO_0001025 rdf:resource="http://purl.obolibrary.org/obo/GAZ_00008123"/>
        <obo:IAO_0000115>A department of Ngounie Province in southern Gabon. The capital lies at Mimongo.</obo:IAO_0000115>
        <oboInOwl:hasOBONamespace>GAZ</oboInOwl:hasOBONamespace>
        <oboInOwl:id>GAZ:00031342</oboInOwl:id>
        <rdfs:label>Ogoulou Department</rdfs:label>
    </owl:NamedIndividual>
    


    <!-- http://purl.obolibrary.org/obo/GAZ_00031343 -->

    <owl:NamedIndividual rdf:about="http://purl.obolibrary.org/obo/GAZ_00031343">
        <obo:RO_0001025 rdf:resource="http://purl.obolibrary.org/obo/GAZ_00008123"/>
        <obo:IAO_0000115>A department of Ngounie Province in south-western Gabon. The capital lies at Mandji.</obo:IAO_0000115>
        <oboInOwl:hasOBONamespace>GAZ</oboInOwl:hasOBONamespace>
        <oboInOwl:id>GAZ:00031343</oboInOwl:id>
        <rdfs:label>Ndolou Department</rdfs:label>
    </owl:NamedIndividual>
    


    <!-- http://purl.obolibrary.org/obo/GAZ_00031344 -->

    <owl:NamedIndividual rdf:about="http://purl.obolibrary.org/obo/GAZ_00031344">
        <obo:RO_0001025 rdf:resource="http://purl.obolibrary.org/obo/GAZ_00008123"/>
        <obo:IAO_0000115>A department of Ngounie Province in southern Gabon. The capital lies at Ndende.</obo:IAO_0000115>
        <oboInOwl:hasOBONamespace>GAZ</oboInOwl:hasOBONamespace>
        <oboInOwl:id>GAZ:00031344</oboInOwl:id>
        <rdfs:label>Dola Department</rdfs:label>
    </owl:NamedIndividual>
    


    <!-- http://purl.obolibrary.org/obo/GAZ_00031345 -->

    <owl:NamedIndividual rdf:about="http://purl.obolibrary.org/obo/GAZ_00031345">
        <obo:RO_0001025 rdf:resource="http://purl.obolibrary.org/obo/GAZ_00008123"/>
        <obo:IAO_0000115>A department of Ngounie Province in south-western Gabon. The capital lies at Lebamba.</obo:IAO_0000115>
        <oboInOwl:hasOBONamespace>GAZ</oboInOwl:hasOBONamespace>
        <oboInOwl:id>GAZ:00031345</oboInOwl:id>
        <rdfs:label>Louetsi-Wano Department</rdfs:label>
    </owl:NamedIndividual>
    


    <!-- http://purl.obolibrary.org/obo/GAZ_00031346 -->

    <owl:NamedIndividual rdf:about="http://purl.obolibrary.org/obo/GAZ_00031346">
        <obo:RO_0001025 rdf:resource="http://purl.obolibrary.org/obo/GAZ_00008123"/>
        <obo:IAO_0000115>A department of Ngounie Province in southern Gabon. The capital lies at Mbigou.</obo:IAO_0000115>
        <oboInOwl:hasOBONamespace>GAZ</oboInOwl:hasOBONamespace>
        <oboInOwl:id>GAZ:00031346</oboInOwl:id>
        <rdfs:label>Boumi-Louetsi Department</rdfs:label>
    </owl:NamedIndividual>
    


    <!-- http://purl.obolibrary.org/obo/GAZ_00031347 -->

    <owl:NamedIndividual rdf:about="http://purl.obolibrary.org/obo/GAZ_00031347">
        <obo:RO_0001025 rdf:resource="http://purl.obolibrary.org/obo/GAZ_00008123"/>
        <obo:IAO_0000115>A department of Ngounie Province in southern Gabon. The capital lies at Fougamou.</obo:IAO_0000115>
        <oboInOwl:hasOBONamespace>GAZ</oboInOwl:hasOBONamespace>
        <oboInOwl:id>GAZ:00031347</oboInOwl:id>
        <rdfs:label>Tsamba-Magotsi Department</rdfs:label>
    </owl:NamedIndividual>
    


    <!-- http://purl.obolibrary.org/obo/GAZ_00031348 -->

    <owl:NamedIndividual rdf:about="http://purl.obolibrary.org/obo/GAZ_00031348">
        <obo:RO_0001025 rdf:resource="http://purl.obolibrary.org/obo/GAZ_00008123"/>
        <obo:IAO_0000115>A department of Ngounie Province in south-western Gabon. The capital lies at Mouila.</obo:IAO_0000115>
        <oboInOwl:hasOBONamespace>GAZ</oboInOwl:hasOBONamespace>
        <oboInOwl:id>GAZ:00031348</oboInOwl:id>
        <rdfs:label>Douya-Onoy Department</rdfs:label>
    </owl:NamedIndividual>
    


    <!-- http://purl.obolibrary.org/obo/GAZ_00031349 -->

    <owl:NamedIndividual rdf:about="http://purl.obolibrary.org/obo/GAZ_00031349">
        <obo:RO_0001025 rdf:resource="http://purl.obolibrary.org/obo/GAZ_00008122"/>
        <obo:IAO_0000115>A department of Haut-Ogooue Province in south-eastern Gabon. The capital lies at Bongoville.</obo:IAO_0000115>
        <oboInOwl:hasOBONamespace>GAZ</oboInOwl:hasOBONamespace>
        <oboInOwl:id>GAZ:00031349</oboInOwl:id>
        <rdfs:label>Djououri-Aguilli Department</rdfs:label>
    </owl:NamedIndividual>
    


    <!-- http://purl.obolibrary.org/obo/GAZ_00031350 -->

    <owl:NamedIndividual rdf:about="http://purl.obolibrary.org/obo/GAZ_00031350">
        <obo:RO_0001025 rdf:resource="http://purl.obolibrary.org/obo/GAZ_00008122"/>
        <obo:IAO_0000115>A department of Haut-Ogooue Province in south-eastern Gabon. The capital lies at Franceville.</obo:IAO_0000115>
        <oboInOwl:hasOBONamespace>GAZ</oboInOwl:hasOBONamespace>
        <oboInOwl:id>GAZ:00031350</oboInOwl:id>
        <rdfs:label>Mpassa Department</rdfs:label>
    </owl:NamedIndividual>
    


    <!-- http://purl.obolibrary.org/obo/GAZ_00031351 -->

    <owl:NamedIndividual rdf:about="http://purl.obolibrary.org/obo/GAZ_00031351">
        <obo:RO_0001025 rdf:resource="http://purl.obolibrary.org/obo/GAZ_00008122"/>
        <obo:IAO_0000115>A department of Haut-Ogooue Province in south-eastern Gabon. The capital lies at Onga.</obo:IAO_0000115>
        <oboInOwl:hasOBONamespace>GAZ</oboInOwl:hasOBONamespace>
        <oboInOwl:id>GAZ:00031351</oboInOwl:id>
        <rdfs:label>Djoue Department</rdfs:label>
    </owl:NamedIndividual>
    


    <!-- http://purl.obolibrary.org/obo/GAZ_00031352 -->

    <owl:NamedIndividual rdf:about="http://purl.obolibrary.org/obo/GAZ_00031352">
        <obo:RO_0001025 rdf:resource="http://purl.obolibrary.org/obo/GAZ_00008122"/>
        <oboInOwl:hasOBONamespace>GAZ</oboInOwl:hasOBONamespace>
        <oboInOwl:id>GAZ:00031352</oboInOwl:id>
        <rdfs:label>Lekoni-Lekori Department</rdfs:label>
    </owl:NamedIndividual>
    


    <!-- http://purl.obolibrary.org/obo/GAZ_00031353 -->

    <owl:NamedIndividual rdf:about="http://purl.obolibrary.org/obo/GAZ_00031353">
        <obo:RO_0001025 rdf:resource="http://purl.obolibrary.org/obo/GAZ_00008122"/>
        <obo:IAO_0000115>A department of Haut-Ogooue Province in eastern Gabon. The capital lies at Okondja.</obo:IAO_0000115>
        <oboInOwl:hasOBONamespace>GAZ</oboInOwl:hasOBONamespace>
        <oboInOwl:id>GAZ:00031353</oboInOwl:id>
        <rdfs:label>Sebe-Brikolo Department</rdfs:label>
    </owl:NamedIndividual>
    


    <!-- http://purl.obolibrary.org/obo/GAZ_00031354 -->

    <owl:NamedIndividual rdf:about="http://purl.obolibrary.org/obo/GAZ_00031354">
        <obo:RO_0001025 rdf:resource="http://purl.obolibrary.org/obo/GAZ_00008122"/>
        <obo:IAO_0000115>A department of Haut-Ogooue Province in south-eastern Gabon. The capital lies at Bakoumba.</obo:IAO_0000115>
        <oboInOwl:hasOBONamespace>GAZ</oboInOwl:hasOBONamespace>
        <oboInOwl:id>GAZ:00031354</oboInOwl:id>
        <rdfs:label>Lekoko Department</rdfs:label>
    </owl:NamedIndividual>
    


    <!-- http://purl.obolibrary.org/obo/GAZ_00031355 -->

    <owl:NamedIndividual rdf:about="http://purl.obolibrary.org/obo/GAZ_00031355">
        <obo:RO_0001025 rdf:resource="http://purl.obolibrary.org/obo/GAZ_00008122"/>
        <obo:IAO_0000115>A department of Haut-Ogooue Province in south-eastern Gabon. The capital lies at Moanda.</obo:IAO_0000115>
        <oboInOwl:hasOBONamespace>GAZ</oboInOwl:hasOBONamespace>
        <oboInOwl:id>GAZ:00031355</oboInOwl:id>
        <rdfs:label>Leboumbi-Leyou Department</rdfs:label>
    </owl:NamedIndividual>
    


    <!-- http://purl.obolibrary.org/obo/GAZ_00031356 -->

    <owl:NamedIndividual rdf:about="http://purl.obolibrary.org/obo/GAZ_00031356">
        <obo:RO_0001025 rdf:resource="http://purl.obolibrary.org/obo/GAZ_00008122"/>
        <obo:IAO_0000115>A department of Haut-Ogooue Province in south-eastern Gabon. Its capital is Leconi.</obo:IAO_0000115>
        <oboInOwl:hasOBONamespace>GAZ</oboInOwl:hasOBONamespace>
        <oboInOwl:id>GAZ:00031356</oboInOwl:id>
        <rdfs:label>Plateaux Department</rdfs:label>
    </owl:NamedIndividual>
    


    <!-- http://purl.obolibrary.org/obo/GAZ_00052686 -->

    <owl:NamedIndividual rdf:about="http://purl.obolibrary.org/obo/GAZ_00052686">
        <obo:RO_0001025 rdf:resource="http://purl.obolibrary.org/obo/GAZ_00031350"/>
    </owl:NamedIndividual>
    


    <!-- http://purl.obolibrary.org/obo/GAZ_00052687 -->

    <owl:NamedIndividual rdf:about="http://purl.obolibrary.org/obo/GAZ_00052687">
        <obo:RO_0001025 rdf:resource="http://purl.obolibrary.org/obo/GAZ_00052686"/>
        <obo:IAO_0000115>A medical research institute.</obo:IAO_0000115>
        <oboInOwl:hasOBONamespace>GAZ</oboInOwl:hasOBONamespace>
        <oboInOwl:id>GAZ:00052687</oboInOwl:id>
        <rdfs:label>Centre international de recherches medicales de Franceville</rdfs:label>
    </owl:NamedIndividual>
    


    <!-- http://purl.obolibrary.org/obo/GAZ_00052688 -->

    <owl:NamedIndividual rdf:about="http://purl.obolibrary.org/obo/GAZ_00052688">
        <rdf:type rdf:resource="http://purl.obolibrary.org/obo/ENVO_00000856"/>
        <obo:RO_0001025 rdf:resource="http://purl.obolibrary.org/obo/GAZ_00005672"/>
    </owl:NamedIndividual>
    


    <!-- http://purl.obolibrary.org/obo/GAZ_00052689 -->

    <owl:NamedIndividual rdf:about="http://purl.obolibrary.org/obo/GAZ_00052689">
        <obo:RO_0001025 rdf:resource="http://purl.obolibrary.org/obo/GAZ_00005670"/>
        <obo:IAO_0000115>A cape N of Libreville.</obo:IAO_0000115>
        <oboInOwl:hasOBONamespace>GAZ</oboInOwl:hasOBONamespace>
        <oboInOwl:id>GAZ:00052689</oboInOwl:id>
        <rdfs:label>Cap Esterias</rdfs:label>
    </owl:NamedIndividual>
    


    <!-- http://purl.obolibrary.org/obo/GAZ_00052690 -->

    <owl:NamedIndividual rdf:about="http://purl.obolibrary.org/obo/GAZ_00052690">
        <obo:RO_0001025 rdf:resource="http://purl.obolibrary.org/obo/GAZ_00008125"/>
    </owl:NamedIndividual>
    


    <!-- http://purl.obolibrary.org/obo/GAZ_00052691 -->

    <owl:NamedIndividual rdf:about="http://purl.obolibrary.org/obo/GAZ_00052691">
        <obo:RO_0001025 rdf:resource="http://purl.obolibrary.org/obo/GAZ_00005672"/>
        <obo:IAO_0000115>A national park located on the equator, near Booue, in the centre of the vast central African forest block, Lope National Park in Gabon is located 350 km to the east of Libreville. Although the terrain is mostly rain forest, in the north the park contains the last remnants of grass savannas created in Central Africa during the last Ice Age, 15,000 years ago. It was the first protected area in Gabon when the Lope-Okanda Wildlife Reserve was created in 1946. In 2007, the Lope-Okanda landscape was added to the World Heritage List.</obo:IAO_0000115>
        <oboInOwl:hasOBONamespace>GAZ</oboInOwl:hasOBONamespace>
        <oboInOwl:id>GAZ:00052691</oboInOwl:id>
        <rdfs:label>Lope National Park</rdfs:label>
    </owl:NamedIndividual>
    


    <!-- http://purl.obolibrary.org/obo/GAZ_00052692 -->

    <owl:NamedIndividual rdf:about="http://purl.obolibrary.org/obo/GAZ_00052692">
        <obo:RO_0001025 rdf:resource="http://purl.obolibrary.org/obo/GAZ_00001092"/>
        <obo:IAO_0000115>A Biosphere Reserve, situated along the banks of the Ivindo River.</obo:IAO_0000115>
        <oboInOwl:hasOBONamespace>GAZ</oboInOwl:hasOBONamespace>
        <oboInOwl:id>GAZ:00052692</oboInOwl:id>
        <rdfs:label>Ipassa-Makokou Reserve</rdfs:label>
    </owl:NamedIndividual>
    


    <!-- http://purl.obolibrary.org/obo/GAZ_00052693 -->

    <owl:NamedIndividual rdf:about="http://purl.obolibrary.org/obo/GAZ_00052693">
        <obo:RO_0001025 rdf:resource="http://purl.obolibrary.org/obo/GAZ_00052692"/>
        <oboInOwl:hasOBONamespace>GAZ</oboInOwl:hasOBONamespace>
        <oboInOwl:id>GAZ:00052693</oboInOwl:id>
        <rdfs:label>Tropical Ecology Research Institute research Station</rdfs:label>
    </owl:NamedIndividual>
    


    <!-- http://purl.obolibrary.org/obo/GAZ_00052694 -->

    <owl:NamedIndividual rdf:about="http://purl.obolibrary.org/obo/GAZ_00052694">
        <obo:RO_0001025 rdf:resource="http://purl.obolibrary.org/obo/GAZ_00005672"/>
    </owl:NamedIndividual>
    


    <!-- http://purl.obolibrary.org/obo/GAZ_00052695 -->

    <owl:NamedIndividual rdf:about="http://purl.obolibrary.org/obo/GAZ_00052695">
        <obo:RO_0001025 rdf:resource="http://purl.obolibrary.org/obo/GAZ_00005668"/>
        <obo:IAO_0000115>A hospital established in order to study major causes of disease burden in the local population. Since its foundation 25 years ago, it has become a leading African research centre, specialising in pathophysiology and treatment of highly prevalent infectious diseases found in sub-Saharan Africa.</obo:IAO_0000115>
        <oboInOwl:hasOBONamespace>GAZ</oboInOwl:hasOBONamespace>
        <oboInOwl:id>GAZ:00052695</oboInOwl:id>
        <rdfs:label>Albert Schweitzer Hospital</rdfs:label>
    </owl:NamedIndividual>
    


    <!-- http://purl.obolibrary.org/obo/GAZ_00052696 -->

    <owl:NamedIndividual rdf:about="http://purl.obolibrary.org/obo/GAZ_00052696">
        <obo:RO_0001025 rdf:resource="http://purl.obolibrary.org/obo/GAZ_00031335"/>
    </owl:NamedIndividual>
    


    <!-- http://purl.obolibrary.org/obo/GAZ_00052697 -->

    <owl:NamedIndividual rdf:about="http://purl.obolibrary.org/obo/GAZ_00052697">
        <obo:RO_0001025 rdf:resource="http://purl.obolibrary.org/obo/GAZ_00052696"/>
        <obo:IAO_0000115>Karst caves.</obo:IAO_0000115>
        <oboInOwl:hasOBONamespace>GAZ</oboInOwl:hasOBONamespace>
        <oboInOwl:id>GAZ:00052697</oboInOwl:id>
        <rdfs:label>Grottes de Lastourville</rdfs:label>
    </owl:NamedIndividual>
    


    <!-- http://purl.obolibrary.org/obo/GAZ_00052699 -->

    <owl:NamedIndividual rdf:about="http://purl.obolibrary.org/obo/GAZ_00052699"/>
    


    <!-- http://purl.obolibrary.org/obo/GAZ_00052700 -->

    <owl:NamedIndividual rdf:about="http://purl.obolibrary.org/obo/GAZ_00052700">
        <obo:RO_0001025 rdf:resource="http://purl.obolibrary.org/obo/GAZ_00052699"/>
        <oboInOwl:hasOBONamespace>GAZ</oboInOwl:hasOBONamespace>
        <oboInOwl:id>GAZ:00052700</oboInOwl:id>
        <rdfs:label>Bongolo American Mission Hospital</rdfs:label>
    </owl:NamedIndividual>
    


    <!-- http://purl.obolibrary.org/obo/GAZ_00052701 -->

    <owl:NamedIndividual rdf:about="http://purl.obolibrary.org/obo/GAZ_00052701">
        <obo:RO_0001025 rdf:resource="http://purl.obolibrary.org/obo/GAZ_00008125"/>
    </owl:NamedIndividual>
    


    <!-- http://purl.obolibrary.org/obo/GAZ_00052703 -->

    <owl:NamedIndividual rdf:about="http://purl.obolibrary.org/obo/GAZ_00052703">
        <obo:RO_0001025 rdf:resource="http://purl.obolibrary.org/obo/GAZ_00008121"/>
        <obo:IAO_0000115>A region that comprises several contiguous protected areas, including the Petit Loango, Monts Doudou, Ouanga Plain and Moukalaba Reserves, and the ex-hunting reserves of Sette-Cama, Iguela and Ngove-Ndogo, situated beside the coast in south-western Gabon, south-east of Port-Gentil.</obo:IAO_0000115>
        <oboInOwl:hasOBONamespace>GAZ</oboInOwl:hasOBONamespace>
        <oboInOwl:id>GAZ:00052703</oboInOwl:id>
        <rdfs:label>Gamba Protected Areas Complex</rdfs:label>
    </owl:NamedIndividual>
    


    <!-- http://purl.obolibrary.org/obo/GAZ_00052704 -->

    <owl:NamedIndividual rdf:about="http://purl.obolibrary.org/obo/GAZ_00052704">
        <obo:RO_0001025 rdf:resource="http://purl.obolibrary.org/obo/GAZ_00052703"/>
        <oboInOwl:hasOBONamespace>GAZ</oboInOwl:hasOBONamespace>
        <oboInOwl:id>GAZ:00052704</oboInOwl:id>
        <rdfs:label>Reserve des Monts Doudou</rdfs:label>
    </owl:NamedIndividual>
    


    <!-- http://purl.obolibrary.org/obo/GAZ_00052705 -->

    <owl:NamedIndividual rdf:about="http://purl.obolibrary.org/obo/GAZ_00052705">
        <rdf:type rdf:resource="http://purl.obolibrary.org/obo/ENVO_00000856"/>
        <obo:RO_0001025 rdf:resource="http://purl.obolibrary.org/obo/GAZ_00031333"/>
    </owl:NamedIndividual>
    


    <!-- http://purl.obolibrary.org/obo/GAZ_00052706 -->

    <owl:NamedIndividual rdf:about="http://purl.obolibrary.org/obo/GAZ_00052706">
        <rdf:type rdf:resource="http://purl.obolibrary.org/obo/ENVO_00000856"/>
        <obo:RO_0001025 rdf:resource="http://purl.obolibrary.org/obo/GAZ_00031337"/>
    </owl:NamedIndividual>
    


    <!-- http://purl.obolibrary.org/obo/GAZ_00052709 -->

    <owl:NamedIndividual rdf:about="http://purl.obolibrary.org/obo/GAZ_00052709">
        <obo:RO_0001025 rdf:resource="http://purl.obolibrary.org/obo/GAZ_00008124"/>
    </owl:NamedIndividual>
    


    <!-- http://purl.obolibrary.org/obo/GAZ_00052715 -->

    <owl:NamedIndividual rdf:about="http://purl.obolibrary.org/obo/GAZ_00052715">
        <rdf:type rdf:resource="http://purl.obolibrary.org/obo/ENVO_00000856"/>
        <obo:RO_0001025 rdf:resource="http://purl.obolibrary.org/obo/GAZ_00031329"/>
    </owl:NamedIndividual>
    


    <!-- http://purl.obolibrary.org/obo/GAZ_00052716 -->

    <owl:NamedIndividual rdf:about="http://purl.obolibrary.org/obo/GAZ_00052716">
        <obo:RO_0001025 rdf:resource="http://purl.obolibrary.org/obo/GAZ_00031350"/>
        <obo:IAO_0000115>A region near the town of Franceville, in the Haut-Ogooue province of the Central African State of Gabon. The discovery in 1972-09 of several natural nuclear fission reactors in the uranium mines situated there has fired the imagination and aroused the curiosity of scientists. There is strong geochemical evidence that the Oklo uranium deposit behaved as a natural nuclear fission reactor in Precambrian times.</obo:IAO_0000115>
        <oboInOwl:hasOBONamespace>GAZ</oboInOwl:hasOBONamespace>
        <oboInOwl:id>GAZ:00052716</oboInOwl:id>
        <rdfs:label>Oklo</rdfs:label>
    </owl:NamedIndividual>
    


    <!-- http://purl.obolibrary.org/obo/GAZ_00052717 -->

    <owl:NamedIndividual rdf:about="http://purl.obolibrary.org/obo/GAZ_00052717">
        <obo:RO_0001025 rdf:resource="http://purl.obolibrary.org/obo/GAZ_00052716"/>
        <obo:IAO_0000115>A mine near the Mouana Mine that is the site of over a dozen precambrian natural nuclear reactors. Secondary enrichment of uranium oxides in cm to meter sized veins moderated by ground water consumed six tons of U235 and elevated temperatures to a few hundred Celsius. Remarkably the non-volatile fission products moved only a few cm in the veins during the last 1.5 billion years.</obo:IAO_0000115>
        <oboInOwl:hasOBONamespace>GAZ</oboInOwl:hasOBONamespace>
        <oboInOwl:id>GAZ:00052717</oboInOwl:id>
        <rdfs:label>Oklo Mine</rdfs:label>
    </owl:NamedIndividual>
    


    <!-- http://purl.obolibrary.org/obo/GAZ_00052718 -->

    <owl:NamedIndividual rdf:about="http://purl.obolibrary.org/obo/GAZ_00052718">
        <obo:RO_0001025 rdf:resource="http://purl.obolibrary.org/obo/GAZ_00052716"/>
        <obo:IAO_0000115>An uranium mine. Possibly the site of another precambrian reactor, in an extension of the Oklo deposit. The last of the Gabon Uranium Mines to close (in 1997).</obo:IAO_0000115>
        <oboInOwl:hasOBONamespace>GAZ</oboInOwl:hasOBONamespace>
        <oboInOwl:id>GAZ:00052718</oboInOwl:id>
        <rdfs:label>Oklobondo Mine</rdfs:label>
    </owl:NamedIndividual>
    


    <!-- http://purl.obolibrary.org/obo/GAZ_00052719 -->

    <owl:NamedIndividual rdf:about="http://purl.obolibrary.org/obo/GAZ_00052719">
        <rdf:type rdf:resource="http://purl.obolibrary.org/obo/ENVO_00000856"/>
        <obo:RO_0001025 rdf:resource="http://purl.obolibrary.org/obo/GAZ_00008121"/>
    </owl:NamedIndividual>
    


    <!-- http://purl.obolibrary.org/obo/GAZ_00052720 -->

    <owl:NamedIndividual rdf:about="http://purl.obolibrary.org/obo/GAZ_00052720">
        <obo:RO_0001025 rdf:resource="http://purl.obolibrary.org/obo/GAZ_00008121"/>
        <obo:IAO_0000115>The delta of the Ogooue River. It is between Point Fetiche in the Bay of Cape Lopez, to 1deg37minS where the southernmost distributary discharges near the mouth of N&apos;Komi (Fenian Vaz) Lagoon, the next most southerly lagoon.</obo:IAO_0000115>
        <oboInOwl:hasOBONamespace>GAZ</oboInOwl:hasOBONamespace>
        <oboInOwl:id>GAZ:00052720</oboInOwl:id>
        <rdfs:label>Ogooue Delta</rdfs:label>
    </owl:NamedIndividual>
    


    <!-- http://purl.obolibrary.org/obo/GAZ_00052721 -->

    <owl:NamedIndividual rdf:about="http://purl.obolibrary.org/obo/GAZ_00052721">
        <obo:RO_0001025 rdf:resource="http://purl.obolibrary.org/obo/GAZ_00052720"/>
        <oboInOwl:hasOBONamespace>GAZ</oboInOwl:hasOBONamespace>
        <oboInOwl:id>GAZ:00052721</oboInOwl:id>
        <rdfs:label>Rabi-Kounga oilfield</rdfs:label>
    </owl:NamedIndividual>
    


    <!-- http://purl.obolibrary.org/obo/GAZ_00052723 -->

    <owl:NamedIndividual rdf:about="http://purl.obolibrary.org/obo/GAZ_00052723">
        <obo:RO_0001025 rdf:resource="http://purl.obolibrary.org/obo/GAZ_00005670"/>
        <obo:IAO_0000115>A cape situated on the Atlantic coast of northwestern Gabon, Africa. Extending south from the larger peninsula that separates the Gabon estuary from Corisco Bay, the cape juts into the mouth of the estuary.</obo:IAO_0000115>
        <oboInOwl:hasOBONamespace>GAZ</oboInOwl:hasOBONamespace>
        <oboInOwl:id>GAZ:00052723</oboInOwl:id>
        <rdfs:label>Saint Clara Cape</rdfs:label>
    </owl:NamedIndividual>
    


    <!-- http://purl.obolibrary.org/obo/GAZ_00052724 -->

    <owl:NamedIndividual rdf:about="http://purl.obolibrary.org/obo/GAZ_00052724">
        <obo:RO_0001025 rdf:resource="http://purl.obolibrary.org/obo/GAZ_00005672"/>
    </owl:NamedIndividual>
    


    <!-- http://purl.obolibrary.org/obo/GAZ_00052725 -->

    <owl:NamedIndividual rdf:about="http://purl.obolibrary.org/obo/GAZ_00052725">
        <rdf:type rdf:resource="http://purl.obolibrary.org/obo/ENVO_00000856"/>
        <obo:RO_0001025 rdf:resource="http://purl.obolibrary.org/obo/GAZ_00031340"/>
    </owl:NamedIndividual>
    


    <!-- http://purl.obolibrary.org/obo/GAZ_00052726 -->

    <owl:NamedIndividual rdf:about="http://purl.obolibrary.org/obo/GAZ_00052726">
        <obo:RO_0001025 rdf:resource="http://purl.obolibrary.org/obo/GAZ_00008124"/>
        <obo:IAO_0000115>A national park in central Gabon. It is a thin tongue of sand in the extreme south of the country, between Mayumba and the Congo border.</obo:IAO_0000115>
        <oboInOwl:hasOBONamespace>GAZ</oboInOwl:hasOBONamespace>
        <oboInOwl:id>GAZ:00052726</oboInOwl:id>
        <rdfs:label>Mayumba National Park</rdfs:label>
    </owl:NamedIndividual>
    


    <!-- http://purl.obolibrary.org/obo/GAZ_00052727 -->

    <owl:NamedIndividual rdf:about="http://purl.obolibrary.org/obo/GAZ_00052727">
        <obo:RO_0001025 rdf:resource="http://purl.obolibrary.org/obo/GAZ_00008122"/>
        <obo:IAO_0000115>A national park in Gabon.</obo:IAO_0000115>
        <oboInOwl:hasOBONamespace>GAZ</oboInOwl:hasOBONamespace>
        <oboInOwl:id>GAZ:00052727</oboInOwl:id>
        <rdfs:label>Moukalaba Doudou National Park</rdfs:label>
    </owl:NamedIndividual>
    


    <!-- http://purl.obolibrary.org/obo/GAZ_00052728 -->

    <owl:NamedIndividual rdf:about="http://purl.obolibrary.org/obo/GAZ_00052728">
        <obo:RO_0001025 rdf:resource="http://purl.obolibrary.org/obo/GAZ_00005670"/>
        <obo:IAO_0000115>A populated place.</obo:IAO_0000115>
        <oboInOwl:hasOBONamespace>GAZ</oboInOwl:hasOBONamespace>
        <oboInOwl:id>GAZ:00052728</oboInOwl:id>
        <rdfs:label>Abenelang</rdfs:label>
    </owl:NamedIndividual>
    


    <!-- http://purl.obolibrary.org/obo/GAZ_00052729 -->

    <owl:NamedIndividual rdf:about="http://purl.obolibrary.org/obo/GAZ_00052729">
        <obo:RO_0001025 rdf:resource="http://purl.obolibrary.org/obo/GAZ_00008126"/>
    </owl:NamedIndividual>
    


    <!-- http://purl.obolibrary.org/obo/GAZ_00052730 -->

    <owl:NamedIndividual rdf:about="http://purl.obolibrary.org/obo/GAZ_00052730">
        <obo:RO_0001025 rdf:resource="http://purl.obolibrary.org/obo/GAZ_00005672"/>
    </owl:NamedIndividual>
    


    <!-- http://purl.obolibrary.org/obo/GAZ_00052731 -->

    <owl:NamedIndividual rdf:about="http://purl.obolibrary.org/obo/GAZ_00052731">
        <obo:RO_0001025 rdf:resource="http://purl.obolibrary.org/obo/GAZ_00008122"/>
    </owl:NamedIndividual>
    


    <!-- http://purl.obolibrary.org/obo/GAZ_00076376 -->

    <owl:NamedIndividual rdf:about="http://purl.obolibrary.org/obo/GAZ_00076376">
        <obo:RO_0001025 rdf:resource="http://purl.obolibrary.org/obo/GAZ_00005670"/>
        <obo:IAO_0000115>One of 13 national parks in Gabon set up in 2002. Akanda National Park is located in the northeast of the country, near Libreville, with coastline along the Mondah and Corisco bays.</obo:IAO_0000115>
        <oboInOwl:hasOBONamespace>GAZ</oboInOwl:hasOBONamespace>
        <oboInOwl:id>GAZ:00076376</oboInOwl:id>
        <rdfs:label>Akanda National Park</rdfs:label>
    </owl:NamedIndividual>
    


    <!-- http://purl.obolibrary.org/obo/GAZ_00076377 -->

    <owl:NamedIndividual rdf:about="http://purl.obolibrary.org/obo/GAZ_00076377">
        <obo:IAO_0000115>Plateaux that are located around the south-east border between the Republic of Congo and Gabon. In the latter, there are found in the Haut-Ogooue Province, while the Plateaux Province name of Congo is taken after them. Several rivers rises in that area, including the Niari River, which flows in Congo, the Ogooue, Mpassa, Ndjoumou, Lekabi and Lekey Rivers which flow in Gabon.</obo:IAO_0000115>
        <oboInOwl:hasOBONamespace>GAZ</oboInOwl:hasOBONamespace>
        <oboInOwl:id>GAZ:00076377</oboInOwl:id>
        <rdfs:label>Bateke Plateau</rdfs:label>
    </owl:NamedIndividual>
    


    <!-- http://purl.obolibrary.org/obo/GAZ_00076378 -->

    <owl:NamedIndividual rdf:about="http://purl.obolibrary.org/obo/GAZ_00076378">
        <obo:RO_0001025 rdf:resource="http://purl.obolibrary.org/obo/GAZ_00076377"/>
        <obo:IAO_0000115>A national park in the Bateke Plateau, southeastern Gabon.</obo:IAO_0000115>
        <oboInOwl:hasOBONamespace>GAZ</oboInOwl:hasOBONamespace>
        <oboInOwl:id>GAZ:00076378</oboInOwl:id>
        <rdfs:label>Bateke Plateau National Park</rdfs:label>
    </owl:NamedIndividual>
    


    <!-- http://purl.obolibrary.org/obo/GAZ_00076380 -->

    <owl:NamedIndividual rdf:about="http://purl.obolibrary.org/obo/GAZ_00076380">
        <obo:IAO_0000115>A national park in central Gabon. It protects rain forest in the Chaillu Massif.</obo:IAO_0000115>
        <oboInOwl:hasOBONamespace>GAZ</oboInOwl:hasOBONamespace>
        <oboInOwl:id>GAZ:00076380</oboInOwl:id>
        <rdfs:label>Parc national des Monts Birougou</rdfs:label>
    </owl:NamedIndividual>
    


    <!-- http://purl.obolibrary.org/obo/GAZ_00076381 -->

    <owl:NamedIndividual rdf:about="http://purl.obolibrary.org/obo/GAZ_00076381">
        <obo:IAO_0000115>A national park in central Gabon. Waka protects over 1,000 km2 of rain forest in the Chaillu Massif.</obo:IAO_0000115>
        <oboInOwl:hasOBONamespace>GAZ</oboInOwl:hasOBONamespace>
        <oboInOwl:id>GAZ:00076381</oboInOwl:id>
        <rdfs:label>Waka National Park</rdfs:label>
    </owl:NamedIndividual>
    


    <!-- http://purl.obolibrary.org/obo/GAZ_00076382 -->

    <owl:NamedIndividual rdf:about="http://purl.obolibrary.org/obo/GAZ_00076382">
        <obo:RO_0001025 rdf:resource="http://purl.obolibrary.org/obo/GAZ_00001092"/>
        <obo:IAO_0000115>Mountains to the NE of Libreville.</obo:IAO_0000115>
        <oboInOwl:hasOBONamespace>GAZ</oboInOwl:hasOBONamespace>
        <oboInOwl:id>GAZ:00076382</oboInOwl:id>
        <rdfs:label>Crystal Mountains</rdfs:label>
    </owl:NamedIndividual>
    


    <!-- http://purl.obolibrary.org/obo/GAZ_00076384 -->

    <owl:NamedIndividual rdf:about="http://purl.obolibrary.org/obo/GAZ_00076384">
        <obo:RO_0001025 rdf:resource="http://purl.obolibrary.org/obo/GAZ_00001092"/>
        <obo:IAO_0000115>A national park in east-central Gabon. It is bisected by the equator. Established 2002.</obo:IAO_0000115>
        <oboInOwl:hasOBONamespace>GAZ</oboInOwl:hasOBONamespace>
        <oboInOwl:id>GAZ:00076384</oboInOwl:id>
        <rdfs:label>Ivindo National Park</rdfs:label>
    </owl:NamedIndividual>
    


    <!-- http://purl.obolibrary.org/obo/GAZ_00076385 -->

    <owl:NamedIndividual rdf:about="http://purl.obolibrary.org/obo/GAZ_00076385">
        <obo:RO_0001025 rdf:resource="http://purl.obolibrary.org/obo/GAZ_00008121"/>
        <obo:IAO_0000115>A national park in western Gabon. It protects diverse coastal habitat, including part of the 220 km2 Iguela Lagoon, the only significant example of a typical western African lagoon system that is protected within a national park.</obo:IAO_0000115>
        <oboInOwl:hasOBONamespace>GAZ</oboInOwl:hasOBONamespace>
        <oboInOwl:id>GAZ:00076385</oboInOwl:id>
        <rdfs:label>Loango National Park</rdfs:label>
    </owl:NamedIndividual>
    


    <!-- http://purl.obolibrary.org/obo/GAZ_00076388 -->

    <owl:NamedIndividual rdf:about="http://purl.obolibrary.org/obo/GAZ_00076388">
        <obo:RO_0001025 rdf:resource="http://purl.obolibrary.org/obo/GAZ_00008126"/>
        <obo:IAO_0000115>A national park in Gabon.</obo:IAO_0000115>
        <oboInOwl:hasOBONamespace>GAZ</oboInOwl:hasOBONamespace>
        <oboInOwl:id>GAZ:00076388</oboInOwl:id>
        <rdfs:label>Minkebe National Park</rdfs:label>
    </owl:NamedIndividual>
    


    <!-- http://purl.obolibrary.org/obo/GAZ_00076389 -->

    <owl:NamedIndividual rdf:about="http://purl.obolibrary.org/obo/GAZ_00076389">
        <obo:RO_0001025 rdf:resource="http://purl.obolibrary.org/obo/GAZ_00005670"/>
        <obo:IAO_0000115>A national park in Gabon.</obo:IAO_0000115>
        <oboInOwl:hasOBONamespace>GAZ</oboInOwl:hasOBONamespace>
        <oboInOwl:id>GAZ:00076389</oboInOwl:id>
        <rdfs:label>Pongara National Park</rdfs:label>
    </owl:NamedIndividual>
    


    <!-- http://purl.obolibrary.org/obo/GAZ_00076390 -->

    <owl:NamedIndividual rdf:about="http://purl.obolibrary.org/obo/GAZ_00076390">
        <obo:RO_0001025 rdf:resource="http://purl.obolibrary.org/obo/GAZ_00001092"/>
        <obo:IAO_0000115>A national park in Gabon.</obo:IAO_0000115>
        <oboInOwl:hasOBONamespace>GAZ</oboInOwl:hasOBONamespace>
        <oboInOwl:id>GAZ:00076390</oboInOwl:id>
        <rdfs:label>Mwangne National Park</rdfs:label>
    </owl:NamedIndividual>
    


    <!-- http://purl.obolibrary.org/obo/GAZ_00146310 -->

    <owl:NamedIndividual rdf:about="http://purl.obolibrary.org/obo/GAZ_00146310">
        <obo:RO_0001025 rdf:resource="http://purl.obolibrary.org/obo/GAZ_00008121"/>
        <obo:IAO_0000115>A coastal lagoon located in the southwestern part of Gabon.</obo:IAO_0000115>
        <oboInOwl:hasOBONamespace>GAZ</oboInOwl:hasOBONamespace>
        <oboInOwl:id>GAZ:00146310</oboInOwl:id>
        <rdfs:label>Ndogo Lagoon</rdfs:label>
    </owl:NamedIndividual>
    


    <!-- http://purl.obolibrary.org/obo/GAZ_00146322 -->

    <owl:NamedIndividual rdf:about="http://purl.obolibrary.org/obo/GAZ_00146322">
        <obo:RO_0001025 rdf:resource="http://purl.obolibrary.org/obo/GAZ_00008121"/>
        <obo:IAO_0000115>A large lagoon on the Atlantic coast of Gabon.</obo:IAO_0000115>
        <oboInOwl:hasOBONamespace>GAZ</oboInOwl:hasOBONamespace>
        <oboInOwl:id>GAZ:00146322</oboInOwl:id>
        <rdfs:label>Fernan Vaz Lagoon</rdfs:label>
    </owl:NamedIndividual>
    


    <!-- http://purl.obolibrary.org/obo/GAZ_00235667 -->

    <owl:NamedIndividual rdf:about="http://purl.obolibrary.org/obo/GAZ_00235667">
        <obo:IAO_0000115>A river in the southern mainland of Equatorial Guinea. It flows southwest from the country&apos;s central plateau, reaching the sea at the estuary of the Muni River.</obo:IAO_0000115>
        <oboInOwl:hasOBONamespace>GAZ</oboInOwl:hasOBONamespace>
        <oboInOwl:id>GAZ:00235667</oboInOwl:id>
        <rdfs:label>Rio Temboni</rdfs:label>
    </owl:NamedIndividual>
    


    <!-- http://purl.obolibrary.org/obo/GAZ_00235675 -->

    <owl:NamedIndividual rdf:about="http://purl.obolibrary.org/obo/GAZ_00235675">
        <obo:RO_0001025 rdf:resource="http://purl.obolibrary.org/obo/GAZ_00005672"/>
        <obo:IAO_0000115>A river that flows from northeast Gabon to the southwest, eventually discharging to the Ogoue River. It has the following tributaries: Djoua, which is also a natural border between Gabon and Congo, Djadie, which flows across Mekambo, Liboumba, whose main tributary is the Lodie River, Mvoung, which flows across Ovan and main tributary is the Kuye River, Oua, Zadia, Bouinandje, Karangoua.</obo:IAO_0000115>
        <oboInOwl:hasOBONamespace>GAZ</oboInOwl:hasOBONamespace>
        <oboInOwl:id>GAZ:00235675</oboInOwl:id>
        <rdfs:label>Ivindo River</rdfs:label>
    </owl:NamedIndividual>
    


    <!-- http://purl.obolibrary.org/obo/GAZ_00235683 -->

    <owl:NamedIndividual rdf:about="http://purl.obolibrary.org/obo/GAZ_00235683">
        <obo:RO_0001025 rdf:resource="http://purl.obolibrary.org/obo/GAZ_00005672"/>
        <obo:IAO_0000115>A populated place.</obo:IAO_0000115>
        <oboInOwl:hasOBONamespace>GAZ</oboInOwl:hasOBONamespace>
        <oboInOwl:id>GAZ:00235683</oboInOwl:id>
        <rdfs:label>Ayem</rdfs:label>
    </owl:NamedIndividual>
    


    <!-- http://purl.obolibrary.org/obo/GAZ_00235684 -->

    <owl:NamedIndividual rdf:about="http://purl.obolibrary.org/obo/GAZ_00235684">
        <obo:RO_0001025 rdf:resource="http://purl.obolibrary.org/obo/GAZ_02000555"/>
        <obo:IAO_0000115>A populated place.</obo:IAO_0000115>
        <oboInOwl:hasOBONamespace>GAZ</oboInOwl:hasOBONamespace>
        <oboInOwl:id>GAZ:00235684</oboInOwl:id>
        <rdfs:label>Ndjole</rdfs:label>
    </owl:NamedIndividual>
    


    <!-- http://purl.obolibrary.org/obo/GAZ_00235685 -->

    <owl:NamedIndividual rdf:about="http://purl.obolibrary.org/obo/GAZ_00235685">
        <obo:RO_0001025 rdf:resource="http://purl.obolibrary.org/obo/GAZ_00008122"/>
        <obo:IAO_0000115>A populated place.</obo:IAO_0000115>
        <oboInOwl:hasOBONamespace>GAZ</oboInOwl:hasOBONamespace>
        <oboInOwl:id>GAZ:00235685</oboInOwl:id>
        <rdfs:label>Maulongo</rdfs:label>
    </owl:NamedIndividual>
    


    <!-- http://purl.obolibrary.org/obo/GAZ_00235686 -->

    <owl:NamedIndividual rdf:about="http://purl.obolibrary.org/obo/GAZ_00235686">
        <obo:RO_0001025 rdf:resource="http://purl.obolibrary.org/obo/GAZ_00008123"/>
        <obo:IAO_0000115>A populated place.</obo:IAO_0000115>
        <oboInOwl:hasOBONamespace>GAZ</oboInOwl:hasOBONamespace>
        <oboInOwl:id>GAZ:00235686</oboInOwl:id>
        <rdfs:label>Mboungou-Mbadouma</rdfs:label>
    </owl:NamedIndividual>
    


    <!-- http://purl.obolibrary.org/obo/GAZ_00235688 -->

    <owl:NamedIndividual rdf:about="http://purl.obolibrary.org/obo/GAZ_00235688">
        <rdf:type rdf:resource="http://purl.obolibrary.org/obo/ENVO_00000856"/>
        <obo:RO_0001025 rdf:resource="http://purl.obolibrary.org/obo/GAZ_00031356"/>
        <obo:IAO_0000115>A populated place. A town in south eastern Gabon, lying east of Bongoville on the Leconi River, surrounded by the Bateke Plateau.</obo:IAO_0000115>
        <oboInOwl:hasOBONamespace>GAZ</oboInOwl:hasOBONamespace>
        <oboInOwl:id>GAZ:00235688</oboInOwl:id>
        <rdfs:label>Lekoni</rdfs:label>
    </owl:NamedIndividual>
    


    <!-- http://purl.obolibrary.org/obo/GAZ_00235689 -->

    <owl:NamedIndividual rdf:about="http://purl.obolibrary.org/obo/GAZ_00235689">
        <obo:RO_0001025 rdf:resource="http://purl.obolibrary.org/obo/GAZ_00235688"/>
        <obo:IAO_0000115>A wildlife and agricultural park in Leconi in south-east Gabon in Africa.</obo:IAO_0000115>
        <oboInOwl:hasOBONamespace>GAZ</oboInOwl:hasOBONamespace>
        <oboInOwl:id>GAZ:00235689</oboInOwl:id>
        <rdfs:label>Leconi Park</rdfs:label>
    </owl:NamedIndividual>
    


    <!-- http://purl.obolibrary.org/obo/GAZ_00235690 -->

    <owl:NamedIndividual rdf:about="http://purl.obolibrary.org/obo/GAZ_00235690">
        <obo:RO_0001025 rdf:resource="http://purl.obolibrary.org/obo/GAZ_00031355"/>
        <obo:IAO_0000115>A populated place.</obo:IAO_0000115>
        <oboInOwl:hasOBONamespace>GAZ</oboInOwl:hasOBONamespace>
        <oboInOwl:id>GAZ:00235690</oboInOwl:id>
        <rdfs:label>Moanda</rdfs:label>
    </owl:NamedIndividual>
    


    <!-- http://purl.obolibrary.org/obo/GAZ_00235703 -->

    <owl:NamedIndividual rdf:about="http://purl.obolibrary.org/obo/GAZ_00235703">
        <obo:RO_0001025 rdf:resource="http://purl.obolibrary.org/obo/GAZ_00031336"/>
        <obo:IAO_0000115>A populated place. It is the capital of Ogooue-Lolo Province in central Gabon. It lies at the confluence of the River Lolo and the River Bouenguidi.</obo:IAO_0000115>
        <oboInOwl:hasOBONamespace>GAZ</oboInOwl:hasOBONamespace>
        <oboInOwl:id>GAZ:00235703</oboInOwl:id>
        <rdfs:label>Koulamoutou</rdfs:label>
    </owl:NamedIndividual>
    


    <!-- http://purl.obolibrary.org/obo/GAZ_00235721 -->

    <owl:NamedIndividual rdf:about="http://purl.obolibrary.org/obo/GAZ_00235721">
        <obo:RO_0001025 rdf:resource="http://purl.obolibrary.org/obo/GAZ_00031345"/>
        <obo:IAO_0000115>A populated place.</obo:IAO_0000115>
        <oboInOwl:hasOBONamespace>GAZ</oboInOwl:hasOBONamespace>
        <oboInOwl:id>GAZ:00235721</oboInOwl:id>
        <rdfs:label>Lebamba</rdfs:label>
    </owl:NamedIndividual>
    


    <!-- http://purl.obolibrary.org/obo/GAZ_00235722 -->

    <owl:NamedIndividual rdf:about="http://purl.obolibrary.org/obo/GAZ_00235722">
        <obo:RO_0001025 rdf:resource="http://purl.obolibrary.org/obo/GAZ_00031346"/>
        <obo:IAO_0000115>A populated place.</obo:IAO_0000115>
        <oboInOwl:hasOBONamespace>GAZ</oboInOwl:hasOBONamespace>
        <oboInOwl:id>GAZ:00235722</oboInOwl:id>
        <rdfs:label>Mbigou</rdfs:label>
    </owl:NamedIndividual>
    


    <!-- http://purl.obolibrary.org/obo/GAZ_00235728 -->

    <owl:NamedIndividual rdf:about="http://purl.obolibrary.org/obo/GAZ_00235728">
        <obo:RO_0001025 rdf:resource="http://purl.obolibrary.org/obo/GAZ_00031353"/>
        <obo:IAO_0000115>A populated place.</obo:IAO_0000115>
        <oboInOwl:hasOBONamespace>GAZ</oboInOwl:hasOBONamespace>
        <oboInOwl:id>GAZ:00235728</oboInOwl:id>
        <rdfs:label>Okandja</rdfs:label>
    </owl:NamedIndividual>
    


    <!-- http://purl.obolibrary.org/obo/GAZ_00235729 -->

    <owl:NamedIndividual rdf:about="http://purl.obolibrary.org/obo/GAZ_00235729">
        <obo:RO_0001025 rdf:resource="http://purl.obolibrary.org/obo/GAZ_00031339"/>
        <obo:IAO_0000115>A populated place. A city in the Nyanga Province of southern Gabon.</obo:IAO_0000115>
        <oboInOwl:hasOBONamespace>GAZ</oboInOwl:hasOBONamespace>
        <oboInOwl:id>GAZ:00235729</oboInOwl:id>
        <rdfs:label>Tchibanga</rdfs:label>
    </owl:NamedIndividual>
    


    <!-- http://purl.obolibrary.org/obo/GAZ_00235730 -->

    <owl:NamedIndividual rdf:about="http://purl.obolibrary.org/obo/GAZ_00235730">
        <obo:RO_0001025 rdf:resource="http://purl.obolibrary.org/obo/GAZ_00008124"/>
        <obo:IAO_0000115>A river. A tributary of the Nyanga River.</obo:IAO_0000115>
        <oboInOwl:hasOBONamespace>GAZ</oboInOwl:hasOBONamespace>
        <oboInOwl:id>GAZ:00235730</oboInOwl:id>
        <rdfs:label>Moukalaba River</rdfs:label>
    </owl:NamedIndividual>
    


    <!-- http://purl.obolibrary.org/obo/GAZ_00235733 -->

    <owl:NamedIndividual rdf:about="http://purl.obolibrary.org/obo/GAZ_00235733">
        <obo:RO_0001025 rdf:resource="http://purl.obolibrary.org/obo/GAZ_00052720"/>
        <oboInOwl:hasOBONamespace>GAZ</oboInOwl:hasOBONamespace>
        <oboInOwl:id>GAZ:00235733</oboInOwl:id>
        <rdfs:label>Mandji Island</rdfs:label>
    </owl:NamedIndividual>
    


    <!-- http://purl.obolibrary.org/obo/GAZ_00235734 -->

    <owl:NamedIndividual rdf:about="http://purl.obolibrary.org/obo/GAZ_00235734">
        <obo:RO_0001025 rdf:resource="http://purl.obolibrary.org/obo/GAZ_02000561"/>
        <obo:IAO_0000115>A peninsula on the coast of west central Africa, in the country of Gabon. It separates the Gulf of Guinea from the South Atlantic Ocean. Lying in the delta of the Ogooue River, it shelters the seaport of Port-Gentil.</obo:IAO_0000115>
        <oboInOwl:hasOBONamespace>GAZ</oboInOwl:hasOBONamespace>
        <oboInOwl:id>GAZ:00235734</oboInOwl:id>
        <rdfs:label>Cape Lopez</rdfs:label>
    </owl:NamedIndividual>
    


    <!-- http://purl.obolibrary.org/obo/GAZ_00235738 -->

    <owl:NamedIndividual rdf:about="http://purl.obolibrary.org/obo/GAZ_00235738">
        <obo:RO_0001025 rdf:resource="http://purl.obolibrary.org/obo/GAZ_00005670"/>
        <obo:RO_0001025 rdf:resource="http://purl.obolibrary.org/obo/GAZ_00076382"/>
        <obo:IAO_0000115>A national park in northwestern Gabon. It is situated in Crystal Mountains, between Equatorial Guinea and the Ogooue River.</obo:IAO_0000115>
        <oboInOwl:hasOBONamespace>GAZ</oboInOwl:hasOBONamespace>
        <oboInOwl:id>GAZ:00235738</oboInOwl:id>
        <rdfs:label>Monts de Cristal National Park</rdfs:label>
    </owl:NamedIndividual>
    


    <!-- http://purl.obolibrary.org/obo/GAZ_00235752 -->

    <owl:NamedIndividual rdf:about="http://purl.obolibrary.org/obo/GAZ_00235752">
        <obo:RO_0001025 rdf:resource="http://purl.obolibrary.org/obo/GAZ_00008121"/>
        <obo:IAO_0000115>A coastal lagoon.</obo:IAO_0000115>
        <oboInOwl:hasOBONamespace>GAZ</oboInOwl:hasOBONamespace>
        <oboInOwl:id>GAZ:00235752</oboInOwl:id>
        <rdfs:label>Lagune Iguela</rdfs:label>
    </owl:NamedIndividual>
    


    <!-- http://purl.obolibrary.org/obo/GAZ_00235753 -->

    <owl:NamedIndividual rdf:about="http://purl.obolibrary.org/obo/GAZ_00235753">
        <obo:RO_0001025 rdf:resource="http://purl.obolibrary.org/obo/GAZ_00008121"/>
        <obo:IAO_0000115>A coastal lagoon.</obo:IAO_0000115>
        <oboInOwl:hasOBONamespace>GAZ</oboInOwl:hasOBONamespace>
        <oboInOwl:id>GAZ:00235753</oboInOwl:id>
        <rdfs:label>Lagune Nkomi</rdfs:label>
    </owl:NamedIndividual>
    


    <!-- http://purl.obolibrary.org/obo/GAZ_00235754 -->

    <owl:NamedIndividual rdf:about="http://purl.obolibrary.org/obo/GAZ_00235754">
        <obo:RO_0001025 rdf:resource="http://purl.obolibrary.org/obo/GAZ_00008124"/>
        <obo:IAO_0000115>A coastal lagoon.</obo:IAO_0000115>
        <oboInOwl:hasOBONamespace>GAZ</oboInOwl:hasOBONamespace>
        <oboInOwl:id>GAZ:00235754</oboInOwl:id>
        <rdfs:label>Lagune Banio</rdfs:label>
    </owl:NamedIndividual>
    


    <!-- http://purl.obolibrary.org/obo/GAZ_00235755 -->

    <owl:NamedIndividual rdf:about="http://purl.obolibrary.org/obo/GAZ_00235755">
        <obo:RO_0001025 rdf:resource="http://purl.obolibrary.org/obo/GAZ_00005667"/>
        <obo:IAO_0000115>A lake.</obo:IAO_0000115>
        <oboInOwl:hasOBONamespace>GAZ</oboInOwl:hasOBONamespace>
        <oboInOwl:id>GAZ:00235755</oboInOwl:id>
        <rdfs:label>Lac Onangue</rdfs:label>
    </owl:NamedIndividual>
    


    <!-- http://purl.obolibrary.org/obo/GAZ_00235756 -->

    <owl:NamedIndividual rdf:about="http://purl.obolibrary.org/obo/GAZ_00235756">
        <obo:RO_0001025 rdf:resource="http://purl.obolibrary.org/obo/GAZ_00005672"/>
        <obo:IAO_0000115>A protected area.</obo:IAO_0000115>
        <oboInOwl:hasOBONamespace>GAZ</oboInOwl:hasOBONamespace>
        <oboInOwl:id>GAZ:00235756</oboInOwl:id>
        <rdfs:label>Parc National de l&apos; Okanda</rdfs:label>
    </owl:NamedIndividual>
    


    <!-- http://purl.obolibrary.org/obo/GAZ_00235757 -->

    <owl:NamedIndividual rdf:about="http://purl.obolibrary.org/obo/GAZ_00235757">
        <obo:RO_0001025 rdf:resource="http://purl.obolibrary.org/obo/GAZ_00005670"/>
        <obo:IAO_0000115>A short wide estuary in the west of Gabon. The capital Libreville has a large port on the north bank of the estuary which collects water from the River Komo and River Ebe. The estuary empties into the Gulf of Guinea.</obo:IAO_0000115>
        <oboInOwl:hasOBONamespace>GAZ</oboInOwl:hasOBONamespace>
        <oboInOwl:id>GAZ:00235757</oboInOwl:id>
        <rdfs:label>Estuaire du Gabon</rdfs:label>
    </owl:NamedIndividual>
    


    <!-- http://purl.obolibrary.org/obo/GAZ_00247146 -->

    <owl:NamedIndividual rdf:about="http://purl.obolibrary.org/obo/GAZ_00247146">
        <obo:IAO_0000115>A river. A tributary of the Sangha River.</obo:IAO_0000115>
        <oboInOwl:hasOBONamespace>GAZ</oboInOwl:hasOBONamespace>
        <oboInOwl:id>GAZ:00247146</oboInOwl:id>
        <rdfs:label>Ekeia River</rdfs:label>
    </owl:NamedIndividual>
    


    <!-- http://purl.obolibrary.org/obo/GAZ_00247771 -->

    <owl:NamedIndividual rdf:about="http://purl.obolibrary.org/obo/GAZ_00247771">
        <obo:IAO_0000115>A river.</obo:IAO_0000115>
        <oboInOwl:hasOBONamespace>GAZ</oboInOwl:hasOBONamespace>
        <oboInOwl:id>GAZ:00247771</oboInOwl:id>
        <rdfs:label>Likouala aux Herbes River</rdfs:label>
    </owl:NamedIndividual>
    


    <!-- http://purl.obolibrary.org/obo/GAZ_00248098 -->

    <owl:NamedIndividual rdf:about="http://purl.obolibrary.org/obo/GAZ_00248098">
        <obo:IAO_0000115>A river discharging to the Rio Muni Estuary.</obo:IAO_0000115>
        <oboInOwl:hasOBONamespace>GAZ</oboInOwl:hasOBONamespace>
        <oboInOwl:id>GAZ:00248098</oboInOwl:id>
        <rdfs:label>Rio Congu</rdfs:label>
    </owl:NamedIndividual>
    


    <!-- http://purl.obolibrary.org/obo/GAZ_00248099 -->

    <owl:NamedIndividual rdf:about="http://purl.obolibrary.org/obo/GAZ_00248099">
        <obo:IAO_0000115>A river discharging to the Rio Muni Estuary.</obo:IAO_0000115>
        <oboInOwl:hasOBONamespace>GAZ</oboInOwl:hasOBONamespace>
        <oboInOwl:id>GAZ:00248099</oboInOwl:id>
        <rdfs:label>Rio Mitong</rdfs:label>
    </owl:NamedIndividual>
    


    <!-- http://purl.obolibrary.org/obo/GAZ_00248102 -->

    <owl:NamedIndividual rdf:about="http://purl.obolibrary.org/obo/GAZ_00248102">
        <obo:IAO_0000115>A river discharging to the Rio Muni Estuary.</obo:IAO_0000115>
        <oboInOwl:hasOBONamespace>GAZ</oboInOwl:hasOBONamespace>
        <oboInOwl:id>GAZ:00248102</oboInOwl:id>
        <rdfs:label>Rio Mandyani</rdfs:label>
    </owl:NamedIndividual>
    


    <!-- http://purl.obolibrary.org/obo/GAZ_00248284 -->

    <owl:NamedIndividual rdf:about="http://purl.obolibrary.org/obo/GAZ_00248284">
        <obo:RO_0001025 rdf:resource="http://purl.obolibrary.org/obo/GAZ_00005670"/>
        <obo:RO_0001025 rdf:resource="http://purl.obolibrary.org/obo/GAZ_00235667"/>
        <obo:IAO_0000115>A river.</obo:IAO_0000115>
        <oboInOwl:hasOBONamespace>GAZ</oboInOwl:hasOBONamespace>
        <oboInOwl:id>GAZ:00248284</oboInOwl:id>
        <rdfs:label>Noya River</rdfs:label>
    </owl:NamedIndividual>
    


    <!-- http://purl.obolibrary.org/obo/GAZ_00248285 -->

    <owl:NamedIndividual rdf:about="http://purl.obolibrary.org/obo/GAZ_00248285">
        <obo:RO_0001025 rdf:resource="http://purl.obolibrary.org/obo/GAZ_00005670"/>
        <obo:IAO_0000115>A bay.</obo:IAO_0000115>
        <oboInOwl:hasOBONamespace>GAZ</oboInOwl:hasOBONamespace>
        <oboInOwl:id>GAZ:00248285</oboInOwl:id>
        <rdfs:label>Baie de Mondah</rdfs:label>
    </owl:NamedIndividual>
    


    <!-- http://purl.obolibrary.org/obo/GAZ_00248287 -->

    <owl:NamedIndividual rdf:about="http://purl.obolibrary.org/obo/GAZ_00248287">
        <obo:RO_0001025 rdf:resource="http://purl.obolibrary.org/obo/GAZ_02000561"/>
        <obo:IAO_0000115>A bay. Enclosed to the W by Cape Lopez.</obo:IAO_0000115>
        <oboInOwl:hasOBONamespace>GAZ</oboInOwl:hasOBONamespace>
        <oboInOwl:id>GAZ:00248287</oboInOwl:id>
        <rdfs:label>Baie du Cap Lopez</rdfs:label>
    </owl:NamedIndividual>
    


    <!-- http://purl.obolibrary.org/obo/GAZ_00248288 -->

    <owl:NamedIndividual rdf:about="http://purl.obolibrary.org/obo/GAZ_00248288">
        <obo:RO_0001025 rdf:resource="http://purl.obolibrary.org/obo/GAZ_00005667"/>
        <obo:IAO_0000115>A lake to the N of the Ogooue River.</obo:IAO_0000115>
        <oboInOwl:hasOBONamespace>GAZ</oboInOwl:hasOBONamespace>
        <oboInOwl:id>GAZ:00248288</oboInOwl:id>
        <rdfs:label>Lac Iwande</rdfs:label>
    </owl:NamedIndividual>
    


    <!-- http://purl.obolibrary.org/obo/GAZ_00248289 -->

    <owl:NamedIndividual rdf:about="http://purl.obolibrary.org/obo/GAZ_00248289">
        <obo:RO_0001025 rdf:resource="http://purl.obolibrary.org/obo/GAZ_00005667"/>
        <oboInOwl:hasOBONamespace>GAZ</oboInOwl:hasOBONamespace>
        <oboInOwl:id>GAZ:00248289</oboInOwl:id>
        <rdfs:label>Lac Ingoyo</rdfs:label>
    </owl:NamedIndividual>
    


    <!-- http://purl.obolibrary.org/obo/GAZ_00248290 -->

    <owl:NamedIndividual rdf:about="http://purl.obolibrary.org/obo/GAZ_00248290">
        <obo:RO_0001025 rdf:resource="http://purl.obolibrary.org/obo/GAZ_00005667"/>
        <oboInOwl:hasOBONamespace>GAZ</oboInOwl:hasOBONamespace>
        <oboInOwl:id>GAZ:00248290</oboInOwl:id>
        <rdfs:label>Lac Gome</rdfs:label>
    </owl:NamedIndividual>
    


    <!-- http://purl.obolibrary.org/obo/GAZ_00248291 -->

    <owl:NamedIndividual rdf:about="http://purl.obolibrary.org/obo/GAZ_00248291">
        <obo:RO_0001025 rdf:resource="http://purl.obolibrary.org/obo/GAZ_00005667"/>
        <oboInOwl:hasOBONamespace>GAZ</oboInOwl:hasOBONamespace>
        <oboInOwl:id>GAZ:00248291</oboInOwl:id>
        <rdfs:label>Lac Loge</rdfs:label>
    </owl:NamedIndividual>
    


    <!-- http://purl.obolibrary.org/obo/GAZ_00248292 -->

    <owl:NamedIndividual rdf:about="http://purl.obolibrary.org/obo/GAZ_00248292">
        <obo:RO_0001025 rdf:resource="http://purl.obolibrary.org/obo/GAZ_00005667"/>
        <oboInOwl:hasOBONamespace>GAZ</oboInOwl:hasOBONamespace>
        <oboInOwl:id>GAZ:00248292</oboInOwl:id>
        <rdfs:label>Lac Ntchonie</rdfs:label>
    </owl:NamedIndividual>
    


    <!-- http://purl.obolibrary.org/obo/GAZ_00248293 -->

    <owl:NamedIndividual rdf:about="http://purl.obolibrary.org/obo/GAZ_00248293">
        <obo:RO_0001025 rdf:resource="http://purl.obolibrary.org/obo/GAZ_00005667"/>
        <oboInOwl:hasOBONamespace>GAZ</oboInOwl:hasOBONamespace>
        <oboInOwl:id>GAZ:00248293</oboInOwl:id>
        <rdfs:label>Lac Igouloue</rdfs:label>
    </owl:NamedIndividual>
    


    <!-- http://purl.obolibrary.org/obo/GAZ_00248294 -->

    <owl:NamedIndividual rdf:about="http://purl.obolibrary.org/obo/GAZ_00248294">
        <obo:RO_0001025 rdf:resource="http://purl.obolibrary.org/obo/GAZ_00005667"/>
        <oboInOwl:hasOBONamespace>GAZ</oboInOwl:hasOBONamespace>
        <oboInOwl:id>GAZ:00248294</oboInOwl:id>
        <rdfs:label>Lac Akombie</rdfs:label>
    </owl:NamedIndividual>
    


    <!-- http://purl.obolibrary.org/obo/GAZ_00248295 -->

    <owl:NamedIndividual rdf:about="http://purl.obolibrary.org/obo/GAZ_00248295">
        <obo:RO_0001025 rdf:resource="http://purl.obolibrary.org/obo/GAZ_00005667"/>
        <oboInOwl:hasOBONamespace>GAZ</oboInOwl:hasOBONamespace>
        <oboInOwl:id>GAZ:00248295</oboInOwl:id>
        <rdfs:label>Lac Nkomie</rdfs:label>
    </owl:NamedIndividual>
    


    <!-- http://purl.obolibrary.org/obo/GAZ_00248296 -->

    <owl:NamedIndividual rdf:about="http://purl.obolibrary.org/obo/GAZ_00248296">
        <obo:RO_0001025 rdf:resource="http://purl.obolibrary.org/obo/GAZ_00005667"/>
        <oboInOwl:hasOBONamespace>GAZ</oboInOwl:hasOBONamespace>
        <oboInOwl:id>GAZ:00248296</oboInOwl:id>
        <rdfs:label>Lac Ogonobie</rdfs:label>
    </owl:NamedIndividual>
    


    <!-- http://purl.obolibrary.org/obo/GAZ_00248297 -->

    <owl:NamedIndividual rdf:about="http://purl.obolibrary.org/obo/GAZ_00248297">
        <obo:RO_0001025 rdf:resource="http://purl.obolibrary.org/obo/GAZ_00005667"/>
        <obo:IAO_0000115>A lake to the S of the Onoogue River.</obo:IAO_0000115>
        <oboInOwl:hasOBONamespace>GAZ</oboInOwl:hasOBONamespace>
        <oboInOwl:id>GAZ:00248297</oboInOwl:id>
        <rdfs:label>Lac Auanga</rdfs:label>
    </owl:NamedIndividual>
    


    <!-- http://purl.obolibrary.org/obo/GAZ_00248298 -->

    <owl:NamedIndividual rdf:about="http://purl.obolibrary.org/obo/GAZ_00248298">
        <obo:RO_0001025 rdf:resource="http://purl.obolibrary.org/obo/GAZ_00005667"/>
        <oboInOwl:hasOBONamespace>GAZ</oboInOwl:hasOBONamespace>
        <oboInOwl:id>GAZ:00248298</oboInOwl:id>
        <rdfs:label>Lac Ogonie</rdfs:label>
    </owl:NamedIndividual>
    


    <!-- http://purl.obolibrary.org/obo/GAZ_00248300 -->

    <owl:NamedIndividual rdf:about="http://purl.obolibrary.org/obo/GAZ_00248300">
        <obo:RO_0001025 rdf:resource="http://purl.obolibrary.org/obo/GAZ_00008121"/>
        <obo:IAO_0000115>A lagoon.</obo:IAO_0000115>
        <oboInOwl:hasOBONamespace>GAZ</oboInOwl:hasOBONamespace>
        <oboInOwl:id>GAZ:00248300</oboInOwl:id>
        <rdfs:label>Lagune Sounga</rdfs:label>
    </owl:NamedIndividual>
    


    <!-- http://purl.obolibrary.org/obo/GAZ_00248301 -->

    <owl:NamedIndividual rdf:about="http://purl.obolibrary.org/obo/GAZ_00248301">
        <obo:RO_0001025 rdf:resource="http://purl.obolibrary.org/obo/GAZ_00008124"/>
        <obo:IAO_0000115>A lake.</obo:IAO_0000115>
        <oboInOwl:hasOBONamespace>GAZ</oboInOwl:hasOBONamespace>
        <oboInOwl:id>GAZ:00248301</oboInOwl:id>
        <rdfs:label>Lac Mandje</rdfs:label>
    </owl:NamedIndividual>
    


    <!-- http://purl.obolibrary.org/obo/GAZ_00248305 -->

    <owl:NamedIndividual rdf:about="http://purl.obolibrary.org/obo/GAZ_00248305">
        <obo:RO_0001025 rdf:resource="http://purl.obolibrary.org/obo/GAZ_00008121"/>
        <obo:IAO_0000115>A protected area. Located betweenLibreville and Port Gentil.</obo:IAO_0000115>
        <oboInOwl:hasOBONamespace>GAZ</oboInOwl:hasOBONamespace>
        <oboInOwl:id>GAZ:00248305</oboInOwl:id>
        <rdfs:label>Reserve de Wonga Wongue</rdfs:label>
    </owl:NamedIndividual>
    


    <!-- http://purl.obolibrary.org/obo/GAZ_00248306 -->

    <owl:NamedIndividual rdf:about="http://purl.obolibrary.org/obo/GAZ_00248306">
        <obo:RO_0001025 rdf:resource="http://purl.obolibrary.org/obo/GAZ_00008121"/>
        <obo:IAO_0000115>A protected area.</obo:IAO_0000115>
        <oboInOwl:hasOBONamespace>GAZ</oboInOwl:hasOBONamespace>
        <oboInOwl:id>GAZ:00248306</oboInOwl:id>
        <rdfs:label>Reserve de Petit-Loango</rdfs:label>
    </owl:NamedIndividual>
    


    <!-- http://purl.obolibrary.org/obo/GAZ_00248307 -->

    <owl:NamedIndividual rdf:about="http://purl.obolibrary.org/obo/GAZ_00248307">
        <obo:RO_0001025 rdf:resource="http://purl.obolibrary.org/obo/GAZ_00008121"/>
        <obo:IAO_0000115>A protected area.</obo:IAO_0000115>
        <oboInOwl:hasOBONamespace>GAZ</oboInOwl:hasOBONamespace>
        <oboInOwl:id>GAZ:00248307</oboInOwl:id>
        <rdfs:label>Reserve de Moukalaba</rdfs:label>
    </owl:NamedIndividual>
    


    <!-- http://purl.obolibrary.org/obo/GAZ_02000554 -->

    <owl:NamedIndividual rdf:about="http://purl.obolibrary.org/obo/GAZ_02000554">
        <obo:RO_0001025 rdf:resource="http://purl.obolibrary.org/obo/GAZ_00005667"/>
        <obo:IAO_0000115>A department of Moyen-Ogooue Province in western Gabon. The capital lies at Lambarene.</obo:IAO_0000115>
        <oboInOwl:hasOBONamespace>GAZ</oboInOwl:hasOBONamespace>
        <oboInOwl:id>GAZ:02000554</oboInOwl:id>
        <rdfs:label>Ogooue et des Lacs Departmenr</rdfs:label>
    </owl:NamedIndividual>
    


    <!-- http://purl.obolibrary.org/obo/GAZ_02000555 -->

    <owl:NamedIndividual rdf:about="http://purl.obolibrary.org/obo/GAZ_02000555">
        <obo:RO_0001025 rdf:resource="http://purl.obolibrary.org/obo/GAZ_00005667"/>
        <obo:IAO_0000115>A department of Moyen-Ogooue Province in western Gabon. The capital lies at Ndjole.</obo:IAO_0000115>
        <oboInOwl:hasOBONamespace>GAZ</oboInOwl:hasOBONamespace>
        <oboInOwl:id>GAZ:02000555</oboInOwl:id>
        <rdfs:label>Abanga-Bigne Department</rdfs:label>
    </owl:NamedIndividual>
    


    <!-- http://purl.obolibrary.org/obo/GAZ_02000556 -->

    <owl:NamedIndividual rdf:about="http://purl.obolibrary.org/obo/GAZ_02000556">
        <obo:RO_0001025 rdf:resource="http://purl.obolibrary.org/obo/GAZ_00005670"/>
        <obo:IAO_0000115>A department of Estuaire Province in western Gabon. The capital lies at Cocobeach.</obo:IAO_0000115>
        <oboInOwl:hasOBONamespace>GAZ</oboInOwl:hasOBONamespace>
        <oboInOwl:id>GAZ:02000556</oboInOwl:id>
        <rdfs:label>Noya Department</rdfs:label>
    </owl:NamedIndividual>
    


    <!-- http://purl.obolibrary.org/obo/GAZ_02000557 -->

    <owl:NamedIndividual rdf:about="http://purl.obolibrary.org/obo/GAZ_02000557">
        <obo:RO_0001025 rdf:resource="http://purl.obolibrary.org/obo/GAZ_00005670"/>
        <obo:IAO_0000115>A department of Estuaire Province in western Gabon. The capital lies at Kango.</obo:IAO_0000115>
        <oboInOwl:hasOBONamespace>GAZ</oboInOwl:hasOBONamespace>
        <oboInOwl:id>GAZ:02000557</oboInOwl:id>
        <rdfs:label>Komo Department</rdfs:label>
    </owl:NamedIndividual>
    


    <!-- http://purl.obolibrary.org/obo/GAZ_02000558 -->

    <owl:NamedIndividual rdf:about="http://purl.obolibrary.org/obo/GAZ_02000558">
        <obo:RO_0001025 rdf:resource="http://purl.obolibrary.org/obo/GAZ_00005670"/>
        <obo:IAO_0000115>A department of Estuaire Province in western Gabon. The capital lies at Ntoum.</obo:IAO_0000115>
        <oboInOwl:hasOBONamespace>GAZ</oboInOwl:hasOBONamespace>
        <oboInOwl:id>GAZ:02000558</oboInOwl:id>
        <rdfs:label>Komo-Mondah Department</rdfs:label>
    </owl:NamedIndividual>
    


    <!-- http://purl.obolibrary.org/obo/GAZ_02000559 -->

    <owl:NamedIndividual rdf:about="http://purl.obolibrary.org/obo/GAZ_02000559">
        <obo:RO_0001025 rdf:resource="http://purl.obolibrary.org/obo/GAZ_00005672"/>
        <obo:IAO_0000115>A department of Ogooue-Ivindo Province in central Gabon. The capital lies at Booue.</obo:IAO_0000115>
        <oboInOwl:hasOBONamespace>GAZ</oboInOwl:hasOBONamespace>
        <oboInOwl:id>GAZ:02000559</oboInOwl:id>
        <rdfs:label>Lope Department</rdfs:label>
    </owl:NamedIndividual>
    


    <!-- http://purl.obolibrary.org/obo/GAZ_02000560 -->

    <owl:NamedIndividual rdf:about="http://purl.obolibrary.org/obo/GAZ_02000560">
        <obo:RO_0001025 rdf:resource="http://purl.obolibrary.org/obo/GAZ_00008121"/>
        <obo:IAO_0000115>A department of Ogooue-Maritime Province in western Gabon. The capital lies at Gamba.</obo:IAO_0000115>
        <oboInOwl:hasOBONamespace>GAZ</oboInOwl:hasOBONamespace>
        <oboInOwl:id>GAZ:02000560</oboInOwl:id>
        <rdfs:label>Ndougou Department</rdfs:label>
    </owl:NamedIndividual>
    


    <!-- http://purl.obolibrary.org/obo/GAZ_02000561 -->

    <owl:NamedIndividual rdf:about="http://purl.obolibrary.org/obo/GAZ_02000561">
        <obo:RO_0001025 rdf:resource="http://purl.obolibrary.org/obo/GAZ_00008121"/>
        <obo:IAO_0000115>A department of Ogooue-Maritime Province in western Gabon. The capital lies at Port-Gentil.</obo:IAO_0000115>
        <oboInOwl:hasOBONamespace>GAZ</oboInOwl:hasOBONamespace>
        <oboInOwl:id>GAZ:02000561</oboInOwl:id>
        <rdfs:label>Bendje Department</rdfs:label>
    </owl:NamedIndividual>
    


    <!-- http://purl.obolibrary.org/obo/GAZ_02000562 -->

    <owl:NamedIndividual rdf:about="http://purl.obolibrary.org/obo/GAZ_02000562">
        <obo:RO_0001025 rdf:resource="http://purl.obolibrary.org/obo/GAZ_00008121"/>
        <obo:IAO_0000115>A department of Ogooue-Maritime Province in western Gabon. The capital lies at Omboue.</obo:IAO_0000115>
        <oboInOwl:hasOBONamespace>GAZ</oboInOwl:hasOBONamespace>
        <oboInOwl:id>GAZ:02000562</oboInOwl:id>
        <rdfs:label>Etimboue Department</rdfs:label>
    </owl:NamedIndividual>
    


    <!-- http://purl.obolibrary.org/obo/GAZ_22223531 -->

    <owl:NamedIndividual rdf:about="http://purl.obolibrary.org/obo/GAZ_22223531">
        <obo:RO_0001025 rdf:resource="http://purl.obolibrary.org/obo/GAZ_02000555"/>
        <obo:IAO_0000115>A populated place.</obo:IAO_0000115>
        <oboInOwl:hasOBONamespace>GAZ</oboInOwl:hasOBONamespace>
        <oboInOwl:id>GAZ:22223531</oboInOwl:id>
        <rdfs:label>Andock</rdfs:label>
    </owl:NamedIndividual>
    


    <!-- http://purl.obolibrary.org/obo/GAZ_22223532 -->

    <owl:NamedIndividual rdf:about="http://purl.obolibrary.org/obo/GAZ_22223532">
        <obo:RO_0001025 rdf:resource="http://purl.obolibrary.org/obo/GAZ_00031330"/>
        <obo:IAO_0000115>A populated place.</obo:IAO_0000115>
        <oboInOwl:hasOBONamespace>GAZ</oboInOwl:hasOBONamespace>
        <oboInOwl:id>GAZ:22223532</oboInOwl:id>
        <rdfs:label>Minkebe</rdfs:label>
    </owl:NamedIndividual>
    


    <!-- http://purl.obolibrary.org/obo/GAZ_22223533 -->

    <owl:NamedIndividual rdf:about="http://purl.obolibrary.org/obo/GAZ_22223533">
        <obo:RO_0001025 rdf:resource="http://purl.obolibrary.org/obo/GAZ_00009927"/>
        <obo:IAO_0000115>A populated place.</obo:IAO_0000115>
        <oboInOwl:hasOBONamespace>GAZ</oboInOwl:hasOBONamespace>
        <oboInOwl:id>GAZ:22223533</oboInOwl:id>
        <rdfs:label>Mendemba</rdfs:label>
    </owl:NamedIndividual>
    


    <!-- http://purl.obolibrary.org/obo/GAZ_22223534 -->

    <owl:NamedIndividual rdf:about="http://purl.obolibrary.org/obo/GAZ_22223534">
        <obo:RO_0001025 rdf:resource="http://purl.obolibrary.org/obo/GAZ_00009927"/>
    </owl:NamedIndividual>
    


    <!-- 
    ///////////////////////////////////////////////////////////////////////////////////////
    //
    // Annotations
    //
    ///////////////////////////////////////////////////////////////////////////////////////
     -->

    <rdf:Description rdf:about="http://purl.obolibrary.org/obo/GAZ_00005666">
        <rdfs:label>Province (Gabon)</rdfs:label>
        <oboInOwl:id>GAZ:00005666</oboInOwl:id>
        <oboInOwl:hasOBONamespace>GAZ</oboInOwl:hasOBONamespace>
    </rdf:Description>
    <rdf:Description rdf:about="http://purl.obolibrary.org/obo/GAZ_00005667">
        <obo:IAO_0000115>A Province of Gabon. The provincial capital is Lambarene.</obo:IAO_0000115>
        <oboInOwl:id>GAZ:00005667</oboInOwl:id>
        <oboInOwl:hasOBONamespace>GAZ</oboInOwl:hasOBONamespace>
        <rdfs:label>Moyen-Ogooue Province</rdfs:label>
    </rdf:Description>
    <rdf:Description rdf:about="http://purl.obolibrary.org/obo/GAZ_00005668">
        <oboInOwl:id>GAZ:00005668</oboInOwl:id>
        <oboInOwl:hasOBONamespace>GAZ</oboInOwl:hasOBONamespace>
        <rdfs:label>Lambarene</rdfs:label>
        <obo:IAO_0000115>A populated place. A town that is the capital of the political district Moyen-Ogooue in Gabon.</obo:IAO_0000115>
    </rdf:Description>
    <rdf:Description rdf:about="http://purl.obolibrary.org/obo/GAZ_00005669">
        <oboInOwl:id>GAZ:00005669</oboInOwl:id>
        <oboInOwl:hasOBONamespace>GAZ</oboInOwl:hasOBONamespace>
        <rdfs:label>populated place, Gabon</rdfs:label>
    </rdf:Description>
    <rdf:Description rdf:about="http://purl.obolibrary.org/obo/GAZ_00005670">
        <rdfs:label>Estuaire Province</rdfs:label>
        <oboInOwl:id>GAZ:00005670</oboInOwl:id>
        <oboInOwl:hasOBONamespace>GAZ</oboInOwl:hasOBONamespace>
        <obo:IAO_0000115>A Province of Gabon.</obo:IAO_0000115>
    </rdf:Description>
    <rdf:Description rdf:about="http://purl.obolibrary.org/obo/GAZ_00005671">
        <rdfs:label>Libreville</rdfs:label>
        <obo:IAO_0000115>The capital and largest city of Gabon. The city is a port on the Komo River, near the Gulf of Guinea.</obo:IAO_0000115>
        <oboInOwl:hasOBONamespace>GAZ</oboInOwl:hasOBONamespace>
        <oboInOwl:id>GAZ:00005671</oboInOwl:id>
    </rdf:Description>
    <rdf:Description rdf:about="http://purl.obolibrary.org/obo/GAZ_00005672">
        <obo:IAO_0000115>A Province of Gabon. The regional capital is Makokou.</obo:IAO_0000115>
        <rdfs:label>Ogooue-Ivindo Province</rdfs:label>
        <oboInOwl:hasOBONamespace>GAZ</oboInOwl:hasOBONamespace>
        <oboInOwl:id>GAZ:00005672</oboInOwl:id>
    </rdf:Description>
    <rdf:Description rdf:about="http://purl.obolibrary.org/obo/GAZ_00005673">
        <oboInOwl:hasOBONamespace>GAZ</oboInOwl:hasOBONamespace>
        <rdfs:label>Makokou</rdfs:label>
        <obo:IAO_0000115>The regional capital of the Ogooue-Ivindo province in Gabon.</obo:IAO_0000115>
        <oboInOwl:id>GAZ:00005673</oboInOwl:id>
    </rdf:Description>
    <rdf:Description rdf:about="http://purl.obolibrary.org/obo/GAZ_00008121">
        <rdfs:label>Ogooue-Maritime Province</rdfs:label>
        <obo:IAO_0000115>A Province of Gabon. The provincial capital is Port-Gentil.</obo:IAO_0000115>
        <oboInOwl:id>GAZ:00008121</oboInOwl:id>
        <oboInOwl:hasOBONamespace>GAZ</oboInOwl:hasOBONamespace>
    </rdf:Description>
    <rdf:Description rdf:about="http://purl.obolibrary.org/obo/GAZ_00008122">
        <oboInOwl:hasOBONamespace>GAZ</oboInOwl:hasOBONamespace>
        <obo:IAO_0000115>A Province of Gabon.</obo:IAO_0000115>
        <oboInOwl:id>GAZ:00008122</oboInOwl:id>
        <rdfs:label>Haut-Ogooue Province</rdfs:label>
    </rdf:Description>
    <rdf:Description rdf:about="http://purl.obolibrary.org/obo/GAZ_00008123">
        <oboInOwl:hasOBONamespace>GAZ</oboInOwl:hasOBONamespace>
        <rdfs:label>Ngounie Province</rdfs:label>
        <oboInOwl:id>GAZ:00008123</oboInOwl:id>
        <obo:IAO_0000115>A Province of Gabon. The provincial capital is Mouila.</obo:IAO_0000115>
    </rdf:Description>
    <rdf:Description rdf:about="http://purl.obolibrary.org/obo/GAZ_00008124">
        <oboInOwl:hasOBONamespace>GAZ</oboInOwl:hasOBONamespace>
        <obo:IAO_0000115>A Province of Gabon. The provincial capital is Tchibanga.</obo:IAO_0000115>
        <oboInOwl:id>GAZ:00008124</oboInOwl:id>
        <rdfs:label>Nyanga Province</rdfs:label>
    </rdf:Description>
    <rdf:Description rdf:about="http://purl.obolibrary.org/obo/GAZ_00008125">
        <oboInOwl:hasOBONamespace>GAZ</oboInOwl:hasOBONamespace>
        <rdfs:label>Ogooue-Lolo Province</rdfs:label>
        <oboInOwl:id>GAZ:00008125</oboInOwl:id>
        <obo:IAO_0000115>A Province of Gabon. The regional capital is Koulamoutou.</obo:IAO_0000115>
    </rdf:Description>
    <rdf:Description rdf:about="http://purl.obolibrary.org/obo/GAZ_00008126">
        <oboInOwl:id>GAZ:00008126</oboInOwl:id>
        <oboInOwl:hasOBONamespace>GAZ</oboInOwl:hasOBONamespace>
        <obo:IAO_0000115>A Province of Gabon. The provincial capital is Oyem.</obo:IAO_0000115>
        <rdfs:label>Woleu-Ntem Province</rdfs:label>
    </rdf:Description>
    <rdf:Description rdf:about="http://purl.obolibrary.org/obo/GAZ_00008127">
        <oboInOwl:id>GAZ:00008127</oboInOwl:id>
        <oboInOwl:hasOBONamespace>GAZ</oboInOwl:hasOBONamespace>
        <rdfs:label>Port Gentil</rdfs:label>
        <obo:IAO_0000115>The second-largest city of Gabon and a leading seaport.</obo:IAO_0000115>
    </rdf:Description>
    <rdf:Description rdf:about="http://purl.obolibrary.org/obo/GAZ_00009929">
        <rdfs:label>Etakangaye</rdfs:label>
        <obo:IAO_0000115>A populated place.</obo:IAO_0000115>
        <oboInOwl:hasOBONamespace>GAZ</oboInOwl:hasOBONamespace>
        <oboInOwl:id>GAZ:00009929</oboInOwl:id>
    </rdf:Description>
    <rdf:Description rdf:about="http://purl.obolibrary.org/obo/GAZ_00009930">
        <rdfs:label>Booue</rdfs:label>
        <oboInOwl:id>GAZ:00009930</oboInOwl:id>
        <oboInOwl:hasOBONamespace>GAZ</oboInOwl:hasOBONamespace>
        <obo:IAO_0000115>A populated place. A town located in Ogooue-Ivindo province, Gabon.</obo:IAO_0000115>
    </rdf:Description>
    <rdf:Description rdf:about="http://purl.obolibrary.org/obo/GAZ_00009931">
        <rdfs:label>Mekambo</rdfs:label>
        <obo:IAO_0000115>A populated place. A small village in on the banks of the Zadie River.</obo:IAO_0000115>
        <oboInOwl:id>GAZ:00009931</oboInOwl:id>
        <oboInOwl:hasOBONamespace>GAZ</oboInOwl:hasOBONamespace>
    </rdf:Description>
    <rdf:Description rdf:about="http://purl.obolibrary.org/obo/GAZ_00009934">
        <oboInOwl:id>GAZ:00009934</oboInOwl:id>
        <rdfs:label>Mbomo</rdfs:label>
        <obo:IAO_0000115>A populated place.</obo:IAO_0000115>
        <oboInOwl:hasOBONamespace>GAZ</oboInOwl:hasOBONamespace>
    </rdf:Description>
    <rdf:Description rdf:about="http://purl.obolibrary.org/obo/GAZ_00052686">
        <rdfs:label>Franceville</rdfs:label>
        <obo:IAO_0000115>A populated place. A city.</obo:IAO_0000115>
        <oboInOwl:hasOBONamespace>GAZ</oboInOwl:hasOBONamespace>
        <oboInOwl:id>GAZ:00052686</oboInOwl:id>
    </rdf:Description>
    <rdf:Description rdf:about="http://purl.obolibrary.org/obo/GAZ_00052688">
        <oboInOwl:hasOBONamespace>GAZ</oboInOwl:hasOBONamespace>
        <rdfs:label>Belinga</rdfs:label>
        <oboInOwl:id>GAZ:00052688</oboInOwl:id>
        <obo:IAO_0000115>A populated place. A town near the Congo-Brazzaville border.</obo:IAO_0000115>
    </rdf:Description>
    <rdf:Description rdf:about="http://purl.obolibrary.org/obo/GAZ_00052690">
        <oboInOwl:id>GAZ:00052690</oboInOwl:id>
        <obo:IAO_0000115>A populated place.</obo:IAO_0000115>
        <rdfs:label>Dienga</rdfs:label>
        <oboInOwl:hasOBONamespace>GAZ</oboInOwl:hasOBONamespace>
    </rdf:Description>
    <rdf:Description rdf:about="http://purl.obolibrary.org/obo/GAZ_00052694">
        <obo:IAO_0000115>A populated place.</obo:IAO_0000115>
        <oboInOwl:id>GAZ:00052694</oboInOwl:id>
        <rdfs:label>Mvadi</rdfs:label>
        <oboInOwl:hasOBONamespace>GAZ</oboInOwl:hasOBONamespace>
    </rdf:Description>
    <rdf:Description rdf:about="http://purl.obolibrary.org/obo/GAZ_00052696">
        <obo:IAO_0000115>A populated place. A city in central Gabon, lying on the River Ogooue, the Trans-Gabon Railway and the N3 road.</obo:IAO_0000115>
        <oboInOwl:hasOBONamespace>GAZ</oboInOwl:hasOBONamespace>
        <rdfs:label>Lastourville</rdfs:label>
        <oboInOwl:id>GAZ:00052696</oboInOwl:id>
    </rdf:Description>
    <rdf:Description rdf:about="http://purl.obolibrary.org/obo/GAZ_00052699">
        <oboInOwl:hasOBONamespace>GAZ</oboInOwl:hasOBONamespace>
        <obo:IAO_0000115>A populated place.</obo:IAO_0000115>
        <oboInOwl:id>GAZ:00052699</oboInOwl:id>
        <rdfs:label>Lebamba</rdfs:label>
    </rdf:Description>
    <rdf:Description rdf:about="http://purl.obolibrary.org/obo/GAZ_00052701">
        <oboInOwl:hasOBONamespace>GAZ</oboInOwl:hasOBONamespace>
        <oboInOwl:id>GAZ:00052701</oboInOwl:id>
        <rdfs:label>Idembe</rdfs:label>
        <obo:IAO_0000115>A populated place.</obo:IAO_0000115>
    </rdf:Description>
    <rdf:Description rdf:about="http://purl.obolibrary.org/obo/GAZ_00052705">
        <rdfs:label>Oyem</rdfs:label>
        <oboInOwl:hasOBONamespace>GAZ</oboInOwl:hasOBONamespace>
        <obo:IAO_0000115>A populated place. A town that is the capital of Woleu-Ntem province in northern Gabon.</obo:IAO_0000115>
        <oboInOwl:id>GAZ:00052705</oboInOwl:id>
    </rdf:Description>
    <rdf:Description rdf:about="http://purl.obolibrary.org/obo/GAZ_00052706">
        <obo:IAO_0000115>A populated place. A town that is the capital of the Mvoung Department.</obo:IAO_0000115>
        <rdfs:label>Ovan</rdfs:label>
        <oboInOwl:hasOBONamespace>GAZ</oboInOwl:hasOBONamespace>
        <oboInOwl:id>GAZ:00052706</oboInOwl:id>
    </rdf:Description>
    <rdf:Description rdf:about="http://purl.obolibrary.org/obo/GAZ_00052709">
        <oboInOwl:id>GAZ:00052709</oboInOwl:id>
        <oboInOwl:hasOBONamespace>GAZ</oboInOwl:hasOBONamespace>
        <obo:IAO_0000115>A populated place.</obo:IAO_0000115>
        <rdfs:label>Mouvanga</rdfs:label>
    </rdf:Description>
    <rdf:Description rdf:about="http://purl.obolibrary.org/obo/GAZ_00052715">
        <oboInOwl:hasOBONamespace>GAZ</oboInOwl:hasOBONamespace>
        <oboInOwl:id>GAZ:00052715</oboInOwl:id>
        <rdfs:label>Mitzic</rdfs:label>
        <obo:IAO_0000115>A populated place. A town located in Woleu-Ntem province, Gabon.</obo:IAO_0000115>
    </rdf:Description>
    <rdf:Description rdf:about="http://purl.obolibrary.org/obo/GAZ_00052719">
        <oboInOwl:hasOBONamespace>GAZ</oboInOwl:hasOBONamespace>
        <rdfs:label>Petit Loango</rdfs:label>
        <oboInOwl:id>GAZ:00052719</oboInOwl:id>
        <obo:IAO_0000115>A populated place. A town located in Ogooue-Maritime province, Gabon.</obo:IAO_0000115>
    </rdf:Description>
    <rdf:Description rdf:about="http://purl.obolibrary.org/obo/GAZ_00052724">
        <rdfs:label>Otouma</rdfs:label>
        <oboInOwl:hasOBONamespace>GAZ</oboInOwl:hasOBONamespace>
        <oboInOwl:id>GAZ:00052724</oboInOwl:id>
        <obo:IAO_0000115>A populated place.</obo:IAO_0000115>
    </rdf:Description>
    <rdf:Description rdf:about="http://purl.obolibrary.org/obo/GAZ_00052725">
        <oboInOwl:hasOBONamespace>GAZ</oboInOwl:hasOBONamespace>
        <oboInOwl:id>GAZ:00052725</oboInOwl:id>
        <rdfs:label>Mayumba</rdfs:label>
        <obo:IAO_0000115>A populated place. A town on the Atlantic Ocean coast of Gabon, at the end of the N6 road, lying on a peninsula separated from the mainland by the Banio Lagoon.</obo:IAO_0000115>
    </rdf:Description>
    <rdf:Description rdf:about="http://purl.obolibrary.org/obo/GAZ_00052729">
        <obo:IAO_0000115>A populated place.</obo:IAO_0000115>
        <rdfs:label>Ebeigne</rdfs:label>
        <oboInOwl:hasOBONamespace>GAZ</oboInOwl:hasOBONamespace>
        <oboInOwl:id>GAZ:00052729</oboInOwl:id>
    </rdf:Description>
    <rdf:Description rdf:about="http://purl.obolibrary.org/obo/GAZ_00052730">
        <rdfs:label>Etakaniabe</rdfs:label>
        <oboInOwl:id>GAZ:00052730</oboInOwl:id>
        <obo:IAO_0000115>A populated place.</obo:IAO_0000115>
        <oboInOwl:hasOBONamespace>GAZ</oboInOwl:hasOBONamespace>
    </rdf:Description>
    <rdf:Description rdf:about="http://purl.obolibrary.org/obo/GAZ_00052731">
        <obo:IAO_0000115>A populated place.</obo:IAO_0000115>
        <rdfs:label>Mopia</rdfs:label>
        <oboInOwl:id>GAZ:00052731</oboInOwl:id>
        <oboInOwl:hasOBONamespace>GAZ</oboInOwl:hasOBONamespace>
    </rdf:Description>
    <rdf:Description rdf:about="http://purl.obolibrary.org/obo/GAZ_22223534">
        <oboInOwl:hasOBONamespace>GAZ</oboInOwl:hasOBONamespace>
        <rdfs:label>Ekata</rdfs:label>
        <oboInOwl:id>GAZ:22223534</oboInOwl:id>
        <obo:IAO_0000115>A populated place. A small village in the northeastern region of Gabon in the province of Ogooue-Ivindo near the Congo border.</obo:IAO_0000115>
    </rdf:Description>
</rdf:RDF>



<!-- Generated by the OWL API (version 4.5.6) https://github.com/owlcs/owlapi -->

