<?xml version="1.0"?>
<rdf:RDF xmlns="http://purl.obolibrary.org/obo/gaz/subsets/countries/Guatemala.owl#"
     xml:base="http://purl.obolibrary.org/obo/gaz/subsets/countries/Guatemala.owl"
     xmlns:dc="http://purl.org/dc/elements/1.1/"
     xmlns:obo="http://purl.obolibrary.org/obo/"
     xmlns:owl="http://www.w3.org/2002/07/owl#"
     xmlns:rdf="http://www.w3.org/1999/02/22-rdf-syntax-ns#"
     xmlns:xml="http://www.w3.org/XML/1998/namespace"
     xmlns:xsd="http://www.w3.org/2001/XMLSchema#"
     xmlns:envo="http://purl.obolibrary.org/obo/envo#"
     xmlns:rdfs="http://www.w3.org/2000/01/rdf-schema#"
     xmlns:oboInOwl="http://www.geneontology.org/formats/oboInOwl#">
    <owl:Ontology rdf:about="http://purl.obolibrary.org/obo/gaz/subsets/countries/Guatemala.owl">
        <owl:imports rdf:resource="http://purl.obolibrary.org/obo/gaz/imports/envo_import.owl"/>
        <owl:imports rdf:resource="http://purl.obolibrary.org/obo/gaz/imports/ro_import.owl"/>
    </owl:Ontology>
    


    <!-- 
    ///////////////////////////////////////////////////////////////////////////////////////
    //
    // Annotation properties
    //
    ///////////////////////////////////////////////////////////////////////////////////////
     -->

    


    <!-- http://purl.obolibrary.org/obo/IAO_0000115 -->

    <owl:AnnotationProperty rdf:about="http://purl.obolibrary.org/obo/IAO_0000115"/>
    


    <!-- http://www.geneontology.org/formats/oboInOwl#hasOBONamespace -->

    <owl:AnnotationProperty rdf:about="http://www.geneontology.org/formats/oboInOwl#hasOBONamespace"/>
    


    <!-- http://www.geneontology.org/formats/oboInOwl#id -->

    <owl:AnnotationProperty rdf:about="http://www.geneontology.org/formats/oboInOwl#id"/>
    


    <!-- 
    ///////////////////////////////////////////////////////////////////////////////////////
    //
    // Object Properties
    //
    ///////////////////////////////////////////////////////////////////////////////////////
     -->

    


    <!-- http://purl.obolibrary.org/obo/RO_0001025 -->

    <owl:ObjectProperty rdf:about="http://purl.obolibrary.org/obo/RO_0001025"/>
    


    <!-- 
    ///////////////////////////////////////////////////////////////////////////////////////
    //
    // Classes
    //
    ///////////////////////////////////////////////////////////////////////////////////////
     -->

    


    <!-- http://purl.obolibrary.org/obo/ENVO_00000009 -->

    <owl:Class rdf:about="http://purl.obolibrary.org/obo/ENVO_00000009"/>
    


    <!-- http://purl.obolibrary.org/obo/ENVO_00000095 -->

    <owl:Class rdf:about="http://purl.obolibrary.org/obo/ENVO_00000095"/>
    


    <!-- http://purl.obolibrary.org/obo/ENVO_00000305 -->

    <owl:Class rdf:about="http://purl.obolibrary.org/obo/ENVO_00000305"/>
    


    <!-- http://purl.obolibrary.org/obo/ENVO_00000856 -->

    <owl:Class rdf:about="http://purl.obolibrary.org/obo/ENVO_00000856"/>
    


    <!-- http://purl.obolibrary.org/obo/GAZ_00000430 -->

    <owl:Class rdf:about="http://purl.obolibrary.org/obo/GAZ_00000430">
        <rdfs:subClassOf rdf:resource="http://purl.obolibrary.org/obo/GAZ_00005152"/>
    </owl:Class>
    


    <!-- http://purl.obolibrary.org/obo/GAZ_00000433 -->

    <owl:Class rdf:about="http://purl.obolibrary.org/obo/GAZ_00000433">
        <rdfs:subClassOf rdf:resource="http://purl.obolibrary.org/obo/GAZ_00005152"/>
    </owl:Class>
    


    <!-- http://purl.obolibrary.org/obo/GAZ_00000439 -->

    <owl:Class rdf:about="http://purl.obolibrary.org/obo/GAZ_00000439">
        <rdfs:subClassOf rdf:resource="http://purl.obolibrary.org/obo/GAZ_00005152"/>
    </owl:Class>
    


    <!-- http://purl.obolibrary.org/obo/GAZ_00000446 -->

    <owl:Class rdf:about="http://purl.obolibrary.org/obo/GAZ_00000446">
        <rdfs:subClassOf rdf:resource="http://purl.obolibrary.org/obo/GAZ_00005152"/>
    </owl:Class>
    


    <!-- http://purl.obolibrary.org/obo/GAZ_00000476 -->

    <owl:Class rdf:about="http://purl.obolibrary.org/obo/GAZ_00000476">
        <rdfs:subClassOf rdf:resource="http://purl.obolibrary.org/obo/GAZ_00005152"/>
    </owl:Class>
    


    <!-- http://purl.obolibrary.org/obo/GAZ_00000477 -->

    <owl:Class rdf:about="http://purl.obolibrary.org/obo/GAZ_00000477">
        <rdfs:subClassOf rdf:resource="http://purl.obolibrary.org/obo/GAZ_00005152"/>
    </owl:Class>
    


    <!-- http://purl.obolibrary.org/obo/GAZ_00000483 -->

    <owl:Class rdf:about="http://purl.obolibrary.org/obo/GAZ_00000483">
        <rdfs:subClassOf rdf:resource="http://purl.obolibrary.org/obo/GAZ_00005152"/>
    </owl:Class>
    


    <!-- http://purl.obolibrary.org/obo/GAZ_00000494 -->

    <owl:Class rdf:about="http://purl.obolibrary.org/obo/GAZ_00000494">
        <rdfs:subClassOf rdf:resource="http://purl.obolibrary.org/obo/GAZ_00005152"/>
    </owl:Class>
    


    <!-- http://purl.obolibrary.org/obo/GAZ_00000496 -->

    <owl:Class rdf:about="http://purl.obolibrary.org/obo/GAZ_00000496">
        <rdfs:subClassOf rdf:resource="http://purl.obolibrary.org/obo/GAZ_00005152"/>
    </owl:Class>
    


    <!-- http://purl.obolibrary.org/obo/GAZ_00000499 -->

    <owl:Class rdf:about="http://purl.obolibrary.org/obo/GAZ_00000499">
        <rdfs:subClassOf rdf:resource="http://purl.obolibrary.org/obo/GAZ_00005152"/>
    </owl:Class>
    


    <!-- http://purl.obolibrary.org/obo/GAZ_00000508 -->

    <owl:Class rdf:about="http://purl.obolibrary.org/obo/GAZ_00000508">
        <rdfs:subClassOf rdf:resource="http://purl.obolibrary.org/obo/GAZ_00005152"/>
    </owl:Class>
    


    <!-- http://purl.obolibrary.org/obo/GAZ_00000510 -->

    <owl:Class rdf:about="http://purl.obolibrary.org/obo/GAZ_00000510">
        <rdfs:subClassOf rdf:resource="http://purl.obolibrary.org/obo/GAZ_00005152"/>
    </owl:Class>
    


    <!-- http://purl.obolibrary.org/obo/GAZ_00000517 -->

    <owl:Class rdf:about="http://purl.obolibrary.org/obo/GAZ_00000517">
        <rdfs:subClassOf rdf:resource="http://purl.obolibrary.org/obo/GAZ_00005152"/>
    </owl:Class>
    


    <!-- http://purl.obolibrary.org/obo/GAZ_00000522 -->

    <owl:Class rdf:about="http://purl.obolibrary.org/obo/GAZ_00000522">
        <rdfs:subClassOf rdf:resource="http://purl.obolibrary.org/obo/GAZ_00005152"/>
    </owl:Class>
    


    <!-- http://purl.obolibrary.org/obo/GAZ_00000525 -->

    <owl:Class rdf:about="http://purl.obolibrary.org/obo/GAZ_00000525">
        <rdfs:subClassOf rdf:resource="http://purl.obolibrary.org/obo/GAZ_00005152"/>
    </owl:Class>
    


    <!-- http://purl.obolibrary.org/obo/GAZ_00000529 -->

    <owl:Class rdf:about="http://purl.obolibrary.org/obo/GAZ_00000529">
        <rdfs:subClassOf rdf:resource="http://purl.obolibrary.org/obo/GAZ_00005152"/>
    </owl:Class>
    


    <!-- http://purl.obolibrary.org/obo/GAZ_00000540 -->

    <owl:Class rdf:about="http://purl.obolibrary.org/obo/GAZ_00000540">
        <rdfs:subClassOf rdf:resource="http://purl.obolibrary.org/obo/GAZ_00005152"/>
    </owl:Class>
    


    <!-- http://purl.obolibrary.org/obo/GAZ_00000541 -->

    <owl:Class rdf:about="http://purl.obolibrary.org/obo/GAZ_00000541">
        <rdfs:subClassOf rdf:resource="http://purl.obolibrary.org/obo/GAZ_00005152"/>
    </owl:Class>
    


    <!-- http://purl.obolibrary.org/obo/GAZ_00000545 -->

    <owl:Class rdf:about="http://purl.obolibrary.org/obo/GAZ_00000545">
        <rdfs:subClassOf rdf:resource="http://purl.obolibrary.org/obo/GAZ_00005152"/>
    </owl:Class>
    


    <!-- http://purl.obolibrary.org/obo/GAZ_00000548 -->

    <owl:Class rdf:about="http://purl.obolibrary.org/obo/GAZ_00000548">
        <rdfs:subClassOf rdf:resource="http://purl.obolibrary.org/obo/GAZ_00005152"/>
    </owl:Class>
    


    <!-- http://purl.obolibrary.org/obo/GAZ_00000549 -->

    <owl:Class rdf:about="http://purl.obolibrary.org/obo/GAZ_00000549">
        <rdfs:subClassOf rdf:resource="http://purl.obolibrary.org/obo/GAZ_00005152"/>
    </owl:Class>
    


    <!-- http://purl.obolibrary.org/obo/GAZ_00005152 -->

    <owl:Class rdf:about="http://purl.obolibrary.org/obo/GAZ_00005152"/>
    


    <!-- http://purl.obolibrary.org/obo/GAZ_00005153 -->

    <owl:Class rdf:about="http://purl.obolibrary.org/obo/GAZ_00005153"/>
    


    <!-- http://purl.obolibrary.org/obo/GAZ_00005154 -->

    <owl:Class rdf:about="http://purl.obolibrary.org/obo/GAZ_00005154">
        <rdfs:subClassOf rdf:resource="http://purl.obolibrary.org/obo/GAZ_00005153"/>
    </owl:Class>
    


    <!-- http://purl.obolibrary.org/obo/GAZ_00005155 -->

    <owl:Class rdf:about="http://purl.obolibrary.org/obo/GAZ_00005155">
        <rdfs:subClassOf rdf:resource="http://purl.obolibrary.org/obo/GAZ_00005152"/>
    </owl:Class>
    


    <!-- http://purl.obolibrary.org/obo/GAZ_00056113 -->

    <owl:Class rdf:about="http://purl.obolibrary.org/obo/GAZ_00056113">
        <rdfs:subClassOf rdf:resource="http://purl.obolibrary.org/obo/GAZ_00005153"/>
    </owl:Class>
    


    <!-- http://purl.obolibrary.org/obo/GAZ_00266012 -->

    <owl:Class rdf:about="http://purl.obolibrary.org/obo/GAZ_00266012">
        <obo:IAO_0000115>A karstic lake in Guatemala. It is located in the middle of a national park covered with tropical rain forest, northwest of Coban, near the border between the departments of Alta Verapaz and El Quiche. The lake is near circular in shape and is probably a cenote or doline.</obo:IAO_0000115>
        <oboInOwl:hasOBONamespace>GAZ</oboInOwl:hasOBONamespace>
        <oboInOwl:id>GAZ:00266012</oboInOwl:id>
        <rdfs:label>Laguna Lachua</rdfs:label>
    </owl:Class>
    


    <!-- 
    ///////////////////////////////////////////////////////////////////////////////////////
    //
    // Individuals
    //
    ///////////////////////////////////////////////////////////////////////////////////////
     -->

    


    <!-- http://purl.obolibrary.org/obo/GAZ_00000430 -->

    <owl:NamedIndividual rdf:about="http://purl.obolibrary.org/obo/GAZ_00000430"/>
    


    <!-- http://purl.obolibrary.org/obo/GAZ_00000431 -->

    <owl:NamedIndividual rdf:about="http://purl.obolibrary.org/obo/GAZ_00000431">
        <rdf:type rdf:resource="http://purl.obolibrary.org/obo/ENVO_00000856"/>
        <obo:RO_0001025 rdf:resource="http://purl.obolibrary.org/obo/GAZ_00000430"/>
        <obo:IAO_0000115>A municipality in the Guatemalan Department of Alta Verapaz.</obo:IAO_0000115>
        <oboInOwl:hasOBONamespace>GAZ</oboInOwl:hasOBONamespace>
        <oboInOwl:id>GAZ:00000431</oboInOwl:id>
        <rdfs:label>Municipality of Panzos</rdfs:label>
    </owl:NamedIndividual>
    


    <!-- http://purl.obolibrary.org/obo/GAZ_00000432 -->

    <owl:NamedIndividual rdf:about="http://purl.obolibrary.org/obo/GAZ_00000432">
        <rdf:type rdf:resource="http://purl.obolibrary.org/obo/ENVO_00000856"/>
        <obo:RO_0001025 rdf:resource="http://purl.obolibrary.org/obo/GAZ_00000430"/>
        <obo:IAO_0000115>A municipality in the Guatemalan department of Alta Verapaz.</obo:IAO_0000115>
        <oboInOwl:hasOBONamespace>GAZ</oboInOwl:hasOBONamespace>
        <oboInOwl:id>GAZ:00000432</oboInOwl:id>
        <rdfs:label>Municipality of San Pedro Carcha</rdfs:label>
    </owl:NamedIndividual>
    


    <!-- http://purl.obolibrary.org/obo/GAZ_00000433 -->

    <owl:NamedIndividual rdf:about="http://purl.obolibrary.org/obo/GAZ_00000433"/>
    


    <!-- http://purl.obolibrary.org/obo/GAZ_00000434 -->

    <owl:NamedIndividual rdf:about="http://purl.obolibrary.org/obo/GAZ_00000434">
        <rdf:type rdf:resource="http://purl.obolibrary.org/obo/ENVO_00000856"/>
        <obo:RO_0001025 rdf:resource="http://purl.obolibrary.org/obo/GAZ_00000433"/>
        <obo:IAO_0000115>A municipality in the Baja Verapaz Department of Guatemala.</obo:IAO_0000115>
        <oboInOwl:hasOBONamespace>GAZ</oboInOwl:hasOBONamespace>
        <oboInOwl:id>GAZ:00000434</oboInOwl:id>
        <rdfs:label>Municipality of Purulha</rdfs:label>
    </owl:NamedIndividual>
    


    <!-- http://purl.obolibrary.org/obo/GAZ_00000435 -->

    <owl:NamedIndividual rdf:about="http://purl.obolibrary.org/obo/GAZ_00000435">
        <rdf:type rdf:resource="http://purl.obolibrary.org/obo/ENVO_00000856"/>
        <obo:RO_0001025 rdf:resource="http://purl.obolibrary.org/obo/GAZ_00000433"/>
        <obo:IAO_0000115>A municipality in the Baja Verapaz Department of Guatemala.</obo:IAO_0000115>
        <oboInOwl:hasOBONamespace>GAZ</oboInOwl:hasOBONamespace>
        <oboInOwl:id>GAZ:00000435</oboInOwl:id>
        <rdfs:label>Municipality of Salama</rdfs:label>
    </owl:NamedIndividual>
    


    <!-- http://purl.obolibrary.org/obo/GAZ_00000436 -->

    <owl:NamedIndividual rdf:about="http://purl.obolibrary.org/obo/GAZ_00000436">
        <obo:RO_0001025 rdf:resource="http://purl.obolibrary.org/obo/GAZ_00000433"/>
        <oboInOwl:hasOBONamespace>GAZ</oboInOwl:hasOBONamespace>
        <oboInOwl:id>GAZ:00000436</oboInOwl:id>
        <rdfs:label>San Sebastian</rdfs:label>
    </owl:NamedIndividual>
    


    <!-- http://purl.obolibrary.org/obo/GAZ_00000438 -->

    <owl:NamedIndividual rdf:about="http://purl.obolibrary.org/obo/GAZ_00000438">
        <obo:RO_0001025 rdf:resource="http://purl.obolibrary.org/obo/GAZ_00000433"/>
        <oboInOwl:hasOBONamespace>GAZ</oboInOwl:hasOBONamespace>
        <oboInOwl:id>GAZ:00000438</oboInOwl:id>
        <rdfs:label>Chisalvador</rdfs:label>
    </owl:NamedIndividual>
    


    <!-- http://purl.obolibrary.org/obo/GAZ_00000439 -->

    <owl:NamedIndividual rdf:about="http://purl.obolibrary.org/obo/GAZ_00000439"/>
    


    <!-- http://purl.obolibrary.org/obo/GAZ_00000440 -->

    <owl:NamedIndividual rdf:about="http://purl.obolibrary.org/obo/GAZ_00000440">
        <rdf:type rdf:resource="http://purl.obolibrary.org/obo/ENVO_00000856"/>
        <obo:RO_0001025 rdf:resource="http://purl.obolibrary.org/obo/GAZ_00000439"/>
        <obo:IAO_0000115>A municipality in the Chimaltenango Department of Guatemala.</obo:IAO_0000115>
        <oboInOwl:hasOBONamespace>GAZ</oboInOwl:hasOBONamespace>
        <oboInOwl:id>GAZ:00000440</oboInOwl:id>
        <rdfs:label>Municipality of Patzun</rdfs:label>
    </owl:NamedIndividual>
    


    <!-- http://purl.obolibrary.org/obo/GAZ_00000441 -->

    <owl:NamedIndividual rdf:about="http://purl.obolibrary.org/obo/GAZ_00000441">
        <rdf:type rdf:resource="http://purl.obolibrary.org/obo/ENVO_00000856"/>
        <obo:RO_0001025 rdf:resource="http://purl.obolibrary.org/obo/GAZ_00000439"/>
        <obo:IAO_0000115>A municipality in the Chimaltenango Department of Guatemala.</obo:IAO_0000115>
        <oboInOwl:hasOBONamespace>GAZ</oboInOwl:hasOBONamespace>
        <oboInOwl:id>GAZ:00000441</oboInOwl:id>
        <rdfs:label>Municipality of Patzicia</rdfs:label>
    </owl:NamedIndividual>
    


    <!-- http://purl.obolibrary.org/obo/GAZ_00000443 -->

    <owl:NamedIndividual rdf:about="http://purl.obolibrary.org/obo/GAZ_00000443">
        <obo:RO_0001025 rdf:resource="http://purl.obolibrary.org/obo/GAZ_00000439"/>
        <obo:IAO_0000115>A populated place.</obo:IAO_0000115>
        <oboInOwl:hasOBONamespace>GAZ</oboInOwl:hasOBONamespace>
        <oboInOwl:id>GAZ:00000443</oboInOwl:id>
        <rdfs:label>La Canoa</rdfs:label>
    </owl:NamedIndividual>
    


    <!-- http://purl.obolibrary.org/obo/GAZ_00000444 -->

    <owl:NamedIndividual rdf:about="http://purl.obolibrary.org/obo/GAZ_00000444">
        <obo:RO_0001025 rdf:resource="http://purl.obolibrary.org/obo/GAZ_00000439"/>
        <oboInOwl:hasOBONamespace>GAZ</oboInOwl:hasOBONamespace>
        <oboInOwl:id>GAZ:00000444</oboInOwl:id>
        <rdfs:label>Nimachun</rdfs:label>
    </owl:NamedIndividual>
    


    <!-- http://purl.obolibrary.org/obo/GAZ_00000445 -->

    <owl:NamedIndividual rdf:about="http://purl.obolibrary.org/obo/GAZ_00000445">
        <obo:RO_0001025 rdf:resource="http://purl.obolibrary.org/obo/GAZ_00000439"/>
        <oboInOwl:hasOBONamespace>GAZ</oboInOwl:hasOBONamespace>
        <oboInOwl:id>GAZ:00000445</oboInOwl:id>
        <rdfs:label>Zabalpop</rdfs:label>
    </owl:NamedIndividual>
    


    <!-- http://purl.obolibrary.org/obo/GAZ_00000446 -->

    <owl:NamedIndividual rdf:about="http://purl.obolibrary.org/obo/GAZ_00000446"/>
    


    <!-- http://purl.obolibrary.org/obo/GAZ_00000447 -->

    <owl:NamedIndividual rdf:about="http://purl.obolibrary.org/obo/GAZ_00000447">
        <rdf:type rdf:resource="http://purl.obolibrary.org/obo/ENVO_00000856"/>
        <obo:RO_0001025 rdf:resource="http://purl.obolibrary.org/obo/GAZ_00000446"/>
        <obo:IAO_0000115>A municipality in the Chiquimula Department of Guatemala.</obo:IAO_0000115>
        <oboInOwl:hasOBONamespace>GAZ</oboInOwl:hasOBONamespace>
        <oboInOwl:id>GAZ:00000447</oboInOwl:id>
        <rdfs:label>Municipality of Ipala</rdfs:label>
    </owl:NamedIndividual>
    


    <!-- http://purl.obolibrary.org/obo/GAZ_00000472 -->

    <owl:NamedIndividual rdf:about="http://purl.obolibrary.org/obo/GAZ_00000472">
        <obo:RO_0001025 rdf:resource="http://purl.obolibrary.org/obo/GAZ_00000446"/>
        <oboInOwl:hasOBONamespace>GAZ</oboInOwl:hasOBONamespace>
        <oboInOwl:id>GAZ:00000472</oboInOwl:id>
        <rdfs:label>Hierbabuena</rdfs:label>
    </owl:NamedIndividual>
    


    <!-- http://purl.obolibrary.org/obo/GAZ_00000473 -->

    <owl:NamedIndividual rdf:about="http://purl.obolibrary.org/obo/GAZ_00000473">
        <obo:RO_0001025 rdf:resource="http://purl.obolibrary.org/obo/GAZ_00000446"/>
        <oboInOwl:hasOBONamespace>GAZ</oboInOwl:hasOBONamespace>
        <oboInOwl:id>GAZ:00000473</oboInOwl:id>
        <rdfs:label>Chiqu</rdfs:label>
    </owl:NamedIndividual>
    


    <!-- http://purl.obolibrary.org/obo/GAZ_00000474 -->

    <owl:NamedIndividual rdf:about="http://purl.obolibrary.org/obo/GAZ_00000474">
        <obo:RO_0001025 rdf:resource="http://purl.obolibrary.org/obo/GAZ_00000446"/>
        <oboInOwl:hasOBONamespace>GAZ</oboInOwl:hasOBONamespace>
        <oboInOwl:id>GAZ:00000474</oboInOwl:id>
        <rdfs:label>Buenavista</rdfs:label>
    </owl:NamedIndividual>
    


    <!-- http://purl.obolibrary.org/obo/GAZ_00000475 -->

    <owl:NamedIndividual rdf:about="http://purl.obolibrary.org/obo/GAZ_00000475">
        <obo:RO_0001025 rdf:resource="http://purl.obolibrary.org/obo/GAZ_00000446"/>
        <obo:IAO_0000115>A populated place.</obo:IAO_0000115>
        <oboInOwl:hasOBONamespace>GAZ</oboInOwl:hasOBONamespace>
        <oboInOwl:id>GAZ:00000475</oboInOwl:id>
        <rdfs:label>Santa Elena</rdfs:label>
    </owl:NamedIndividual>
    


    <!-- http://purl.obolibrary.org/obo/GAZ_00000476 -->

    <owl:NamedIndividual rdf:about="http://purl.obolibrary.org/obo/GAZ_00000476"/>
    


    <!-- http://purl.obolibrary.org/obo/GAZ_00000477 -->

    <owl:NamedIndividual rdf:about="http://purl.obolibrary.org/obo/GAZ_00000477"/>
    


    <!-- http://purl.obolibrary.org/obo/GAZ_00000478 -->

    <owl:NamedIndividual rdf:about="http://purl.obolibrary.org/obo/GAZ_00000478">
        <rdf:type rdf:resource="http://purl.obolibrary.org/obo/ENVO_00000856"/>
        <obo:RO_0001025 rdf:resource="http://purl.obolibrary.org/obo/GAZ_00005155"/>
        <obo:IAO_0000115>A municipality in the Guatemala Department of Guatemala.</obo:IAO_0000115>
        <oboInOwl:hasOBONamespace>GAZ</oboInOwl:hasOBONamespace>
        <oboInOwl:id>GAZ:00000478</oboInOwl:id>
        <rdfs:label>Municipality of Mixco</rdfs:label>
    </owl:NamedIndividual>
    


    <!-- http://purl.obolibrary.org/obo/GAZ_00000479 -->

    <owl:NamedIndividual rdf:about="http://purl.obolibrary.org/obo/GAZ_00000479">
        <rdf:type rdf:resource="http://purl.obolibrary.org/obo/ENVO_00000856"/>
        <obo:RO_0001025 rdf:resource="http://purl.obolibrary.org/obo/GAZ_00005155"/>
        <obo:IAO_0000115>A municipality in the Guatemala Department of Guatemala.</obo:IAO_0000115>
        <oboInOwl:hasOBONamespace>GAZ</oboInOwl:hasOBONamespace>
        <oboInOwl:id>GAZ:00000479</oboInOwl:id>
        <rdfs:label>Municipality of Palencia</rdfs:label>
    </owl:NamedIndividual>
    


    <!-- http://purl.obolibrary.org/obo/GAZ_00000480 -->

    <owl:NamedIndividual rdf:about="http://purl.obolibrary.org/obo/GAZ_00000480">
        <rdf:type rdf:resource="http://purl.obolibrary.org/obo/ENVO_00000856"/>
        <obo:RO_0001025 rdf:resource="http://purl.obolibrary.org/obo/GAZ_00005155"/>
        <obo:IAO_0000115>A municipality in the Guatemala Department of Guatemala.</obo:IAO_0000115>
        <oboInOwl:hasOBONamespace>GAZ</oboInOwl:hasOBONamespace>
        <oboInOwl:id>GAZ:00000480</oboInOwl:id>
        <rdfs:label>Municipality of San Juan Sacatepequez</rdfs:label>
    </owl:NamedIndividual>
    


    <!-- http://purl.obolibrary.org/obo/GAZ_00000481 -->

    <owl:NamedIndividual rdf:about="http://purl.obolibrary.org/obo/GAZ_00000481">
        <rdf:type rdf:resource="http://purl.obolibrary.org/obo/ENVO_00000856"/>
        <obo:RO_0001025 rdf:resource="http://purl.obolibrary.org/obo/GAZ_00005155"/>
        <obo:IAO_0000115>A municipality in the Guatemala Department of Guatemala.</obo:IAO_0000115>
        <oboInOwl:hasOBONamespace>GAZ</oboInOwl:hasOBONamespace>
        <oboInOwl:id>GAZ:00000481</oboInOwl:id>
        <rdfs:label>Municipality of San Raymundo</rdfs:label>
    </owl:NamedIndividual>
    


    <!-- http://purl.obolibrary.org/obo/GAZ_00000482 -->

    <owl:NamedIndividual rdf:about="http://purl.obolibrary.org/obo/GAZ_00000482">
        <obo:RO_0001025 rdf:resource="http://purl.obolibrary.org/obo/GAZ_00005155"/>
        <oboInOwl:hasOBONamespace>GAZ</oboInOwl:hasOBONamespace>
        <oboInOwl:id>GAZ:00000482</oboInOwl:id>
        <rdfs:label>El Rosario</rdfs:label>
    </owl:NamedIndividual>
    


    <!-- http://purl.obolibrary.org/obo/GAZ_00000483 -->

    <owl:NamedIndividual rdf:about="http://purl.obolibrary.org/obo/GAZ_00000483"/>
    


    <!-- http://purl.obolibrary.org/obo/GAZ_00000484 -->

    <owl:NamedIndividual rdf:about="http://purl.obolibrary.org/obo/GAZ_00000484">
        <rdf:type rdf:resource="http://purl.obolibrary.org/obo/ENVO_00000856"/>
        <obo:RO_0001025 rdf:resource="http://purl.obolibrary.org/obo/GAZ_00000483"/>
        <obo:IAO_0000115>A municipality in the Guatemalan Department of Huehuetenango.</obo:IAO_0000115>
        <oboInOwl:hasOBONamespace>GAZ</oboInOwl:hasOBONamespace>
        <oboInOwl:id>GAZ:00000484</oboInOwl:id>
        <rdfs:label>Municipality of San Antonio Huista</rdfs:label>
    </owl:NamedIndividual>
    


    <!-- http://purl.obolibrary.org/obo/GAZ_00000485 -->

    <owl:NamedIndividual rdf:about="http://purl.obolibrary.org/obo/GAZ_00000485">
        <rdf:type rdf:resource="http://purl.obolibrary.org/obo/ENVO_00000856"/>
        <obo:RO_0001025 rdf:resource="http://purl.obolibrary.org/obo/GAZ_00000483"/>
        <obo:IAO_0000115>A municipality in the Guatemalan Department of Huehuetenango.</obo:IAO_0000115>
        <oboInOwl:hasOBONamespace>GAZ</oboInOwl:hasOBONamespace>
        <oboInOwl:id>GAZ:00000485</oboInOwl:id>
        <rdfs:label>Municipality of Jacaltenango</rdfs:label>
    </owl:NamedIndividual>
    


    <!-- http://purl.obolibrary.org/obo/GAZ_00000486 -->

    <owl:NamedIndividual rdf:about="http://purl.obolibrary.org/obo/GAZ_00000486">
        <rdf:type rdf:resource="http://purl.obolibrary.org/obo/ENVO_00000856"/>
        <obo:RO_0001025 rdf:resource="http://purl.obolibrary.org/obo/GAZ_00000483"/>
        <obo:IAO_0000115>A municipality in the Guatemalan Department of Huehuetenango.</obo:IAO_0000115>
        <oboInOwl:hasOBONamespace>GAZ</oboInOwl:hasOBONamespace>
        <oboInOwl:id>GAZ:00000486</oboInOwl:id>
        <rdfs:label>Municipality of Colotenango</rdfs:label>
    </owl:NamedIndividual>
    


    <!-- http://purl.obolibrary.org/obo/GAZ_00000487 -->

    <owl:NamedIndividual rdf:about="http://purl.obolibrary.org/obo/GAZ_00000487">
        <rdf:type rdf:resource="http://purl.obolibrary.org/obo/ENVO_00000856"/>
        <obo:RO_0001025 rdf:resource="http://purl.obolibrary.org/obo/GAZ_00000483"/>
        <obo:IAO_0000115>A municipality in the Guatemalan Department of Huehuetenango.</obo:IAO_0000115>
        <oboInOwl:hasOBONamespace>GAZ</oboInOwl:hasOBONamespace>
        <oboInOwl:id>GAZ:00000487</oboInOwl:id>
        <rdfs:label>Municipality of Malacatancito</rdfs:label>
    </owl:NamedIndividual>
    


    <!-- http://purl.obolibrary.org/obo/GAZ_00000488 -->

    <owl:NamedIndividual rdf:about="http://purl.obolibrary.org/obo/GAZ_00000488">
        <rdf:type rdf:resource="http://purl.obolibrary.org/obo/ENVO_00000856"/>
        <obo:RO_0001025 rdf:resource="http://purl.obolibrary.org/obo/GAZ_00000483"/>
        <obo:IAO_0000115>A municipality in the Guatemalan Department of Huehuetenango.</obo:IAO_0000115>
        <oboInOwl:hasOBONamespace>GAZ</oboInOwl:hasOBONamespace>
        <oboInOwl:id>GAZ:00000488</oboInOwl:id>
        <rdfs:label>Municipality of San Sebastian Huehuetenango</rdfs:label>
    </owl:NamedIndividual>
    


    <!-- http://purl.obolibrary.org/obo/GAZ_00000489 -->

    <owl:NamedIndividual rdf:about="http://purl.obolibrary.org/obo/GAZ_00000489">
        <rdf:type rdf:resource="http://purl.obolibrary.org/obo/ENVO_00000856"/>
        <obo:RO_0001025 rdf:resource="http://purl.obolibrary.org/obo/GAZ_00000483"/>
        <obo:IAO_0000115>A municipality in the Guatemalan Department of Huehuetenango.</obo:IAO_0000115>
        <oboInOwl:hasOBONamespace>GAZ</oboInOwl:hasOBONamespace>
        <oboInOwl:id>GAZ:00000489</oboInOwl:id>
        <rdfs:label>Municipality of San Juan Ixcoy</rdfs:label>
    </owl:NamedIndividual>
    


    <!-- http://purl.obolibrary.org/obo/GAZ_00000490 -->

    <owl:NamedIndividual rdf:about="http://purl.obolibrary.org/obo/GAZ_00000490">
        <rdf:type rdf:resource="http://purl.obolibrary.org/obo/ENVO_00000856"/>
        <obo:RO_0001025 rdf:resource="http://purl.obolibrary.org/obo/GAZ_00000483"/>
        <obo:IAO_0000115>A municipality in the Guatemalan Department of Huehuetenango.</obo:IAO_0000115>
        <oboInOwl:hasOBONamespace>GAZ</oboInOwl:hasOBONamespace>
        <oboInOwl:id>GAZ:00000490</oboInOwl:id>
        <rdfs:label>Municipality of Todos Santos Cuchumatan</rdfs:label>
    </owl:NamedIndividual>
    


    <!-- http://purl.obolibrary.org/obo/GAZ_00000491 -->

    <owl:NamedIndividual rdf:about="http://purl.obolibrary.org/obo/GAZ_00000491">
        <obo:RO_0001025 rdf:resource="http://purl.obolibrary.org/obo/GAZ_00000483"/>
        <oboInOwl:hasOBONamespace>GAZ</oboInOwl:hasOBONamespace>
        <oboInOwl:id>GAZ:00000491</oboInOwl:id>
        <rdfs:label>Extenam</rdfs:label>
    </owl:NamedIndividual>
    


    <!-- http://purl.obolibrary.org/obo/GAZ_00000492 -->

    <owl:NamedIndividual rdf:about="http://purl.obolibrary.org/obo/GAZ_00000492">
        <obo:RO_0001025 rdf:resource="http://purl.obolibrary.org/obo/GAZ_00000483"/>
        <oboInOwl:hasOBONamespace>GAZ</oboInOwl:hasOBONamespace>
        <oboInOwl:id>GAZ:00000492</oboInOwl:id>
        <rdfs:label>Defonso Ixtahua</rdfs:label>
    </owl:NamedIndividual>
    


    <!-- http://purl.obolibrary.org/obo/GAZ_00000493 -->

    <owl:NamedIndividual rdf:about="http://purl.obolibrary.org/obo/GAZ_00000493">
        <obo:RO_0001025 rdf:resource="http://purl.obolibrary.org/obo/GAZ_00000483"/>
        <obo:IAO_0000115>A populated place.</obo:IAO_0000115>
        <oboInOwl:hasOBONamespace>GAZ</oboInOwl:hasOBONamespace>
        <oboInOwl:id>GAZ:00000493</oboInOwl:id>
        <rdfs:label>San Lorenzo</rdfs:label>
    </owl:NamedIndividual>
    


    <!-- http://purl.obolibrary.org/obo/GAZ_00000494 -->

    <owl:NamedIndividual rdf:about="http://purl.obolibrary.org/obo/GAZ_00000494"/>
    


    <!-- http://purl.obolibrary.org/obo/GAZ_00000495 -->

    <owl:NamedIndividual rdf:about="http://purl.obolibrary.org/obo/GAZ_00000495">
        <rdf:type rdf:resource="http://purl.obolibrary.org/obo/ENVO_00000856"/>
        <obo:RO_0001025 rdf:resource="http://purl.obolibrary.org/obo/GAZ_00000494"/>
        <obo:IAO_0000115>A municipality in the Izabal Department of Guatemala.</obo:IAO_0000115>
        <oboInOwl:hasOBONamespace>GAZ</oboInOwl:hasOBONamespace>
        <oboInOwl:id>GAZ:00000495</oboInOwl:id>
        <rdfs:label>Municipality of Morales</rdfs:label>
    </owl:NamedIndividual>
    


    <!-- http://purl.obolibrary.org/obo/GAZ_00000496 -->

    <owl:NamedIndividual rdf:about="http://purl.obolibrary.org/obo/GAZ_00000496"/>
    


    <!-- http://purl.obolibrary.org/obo/GAZ_00000497 -->

    <owl:NamedIndividual rdf:about="http://purl.obolibrary.org/obo/GAZ_00000497">
        <rdf:type rdf:resource="http://purl.obolibrary.org/obo/ENVO_00000856"/>
        <obo:RO_0001025 rdf:resource="http://purl.obolibrary.org/obo/GAZ_00000496"/>
        <obo:IAO_0000115>A municipality in the Jalapa Department of Guatemala.</obo:IAO_0000115>
        <oboInOwl:hasOBONamespace>GAZ</oboInOwl:hasOBONamespace>
        <oboInOwl:id>GAZ:00000497</oboInOwl:id>
        <rdfs:label>Municipality of Mataquescuintla</rdfs:label>
    </owl:NamedIndividual>
    


    <!-- http://purl.obolibrary.org/obo/GAZ_00000498 -->

    <owl:NamedIndividual rdf:about="http://purl.obolibrary.org/obo/GAZ_00000498">
        <rdf:type rdf:resource="http://purl.obolibrary.org/obo/ENVO_00000856"/>
        <obo:RO_0001025 rdf:resource="http://purl.obolibrary.org/obo/GAZ_00000496"/>
        <obo:IAO_0000115>A municipality in the Jalapa Department of Guatemala.</obo:IAO_0000115>
        <oboInOwl:hasOBONamespace>GAZ</oboInOwl:hasOBONamespace>
        <oboInOwl:id>GAZ:00000498</oboInOwl:id>
        <rdfs:label>Municipality of Monjas</rdfs:label>
    </owl:NamedIndividual>
    


    <!-- http://purl.obolibrary.org/obo/GAZ_00000499 -->

    <owl:NamedIndividual rdf:about="http://purl.obolibrary.org/obo/GAZ_00000499"/>
    


    <!-- http://purl.obolibrary.org/obo/GAZ_00000500 -->

    <owl:NamedIndividual rdf:about="http://purl.obolibrary.org/obo/GAZ_00000500">
        <rdf:type rdf:resource="http://purl.obolibrary.org/obo/ENVO_00000856"/>
        <obo:RO_0001025 rdf:resource="http://purl.obolibrary.org/obo/GAZ_00000499"/>
        <obo:IAO_0000115>A municipality in the Jutiapa Department of Guatemala.</obo:IAO_0000115>
        <oboInOwl:hasOBONamespace>GAZ</oboInOwl:hasOBONamespace>
        <oboInOwl:id>GAZ:00000500</oboInOwl:id>
        <rdfs:label>Municipality of Aqua Blanca</rdfs:label>
    </owl:NamedIndividual>
    


    <!-- http://purl.obolibrary.org/obo/GAZ_00000501 -->

    <owl:NamedIndividual rdf:about="http://purl.obolibrary.org/obo/GAZ_00000501">
        <rdf:type rdf:resource="http://purl.obolibrary.org/obo/ENVO_00000856"/>
        <obo:RO_0001025 rdf:resource="http://purl.obolibrary.org/obo/GAZ_00000499"/>
        <obo:IAO_0000115>A municipality in the Jutiapa Department of Guatemala.</obo:IAO_0000115>
        <oboInOwl:hasOBONamespace>GAZ</oboInOwl:hasOBONamespace>
        <oboInOwl:id>GAZ:00000501</oboInOwl:id>
        <rdfs:label>Municipality of Asuncion Mita</rdfs:label>
    </owl:NamedIndividual>
    


    <!-- http://purl.obolibrary.org/obo/GAZ_00000502 -->

    <owl:NamedIndividual rdf:about="http://purl.obolibrary.org/obo/GAZ_00000502">
        <rdf:type rdf:resource="http://purl.obolibrary.org/obo/ENVO_00000856"/>
        <obo:RO_0001025 rdf:resource="http://purl.obolibrary.org/obo/GAZ_00000499"/>
        <obo:IAO_0000115>A municipality in the Jutiapa Department of Guatemala.</obo:IAO_0000115>
        <oboInOwl:hasOBONamespace>GAZ</oboInOwl:hasOBONamespace>
        <oboInOwl:id>GAZ:00000502</oboInOwl:id>
        <rdfs:label>Municipality of El Progreso</rdfs:label>
    </owl:NamedIndividual>
    


    <!-- http://purl.obolibrary.org/obo/GAZ_00000503 -->

    <owl:NamedIndividual rdf:about="http://purl.obolibrary.org/obo/GAZ_00000503">
        <rdf:type rdf:resource="http://purl.obolibrary.org/obo/ENVO_00000856"/>
        <obo:RO_0001025 rdf:resource="http://purl.obolibrary.org/obo/GAZ_00000499"/>
        <obo:IAO_0000115>A municipality in the Jutiapa Department of Guatemala.</obo:IAO_0000115>
        <oboInOwl:hasOBONamespace>GAZ</oboInOwl:hasOBONamespace>
        <oboInOwl:id>GAZ:00000503</oboInOwl:id>
        <rdfs:label>Municipality of Jutiapa</rdfs:label>
    </owl:NamedIndividual>
    


    <!-- http://purl.obolibrary.org/obo/GAZ_00000504 -->

    <owl:NamedIndividual rdf:about="http://purl.obolibrary.org/obo/GAZ_00000504">
        <rdf:type rdf:resource="http://purl.obolibrary.org/obo/ENVO_00000856"/>
        <obo:RO_0001025 rdf:resource="http://purl.obolibrary.org/obo/GAZ_00000499"/>
        <obo:IAO_0000115>A municipality in the Jutiapa Department of Guatemala.</obo:IAO_0000115>
        <oboInOwl:hasOBONamespace>GAZ</oboInOwl:hasOBONamespace>
        <oboInOwl:id>GAZ:00000504</oboInOwl:id>
        <rdfs:label>Municipality of Quezada</rdfs:label>
    </owl:NamedIndividual>
    


    <!-- http://purl.obolibrary.org/obo/GAZ_00000505 -->

    <owl:NamedIndividual rdf:about="http://purl.obolibrary.org/obo/GAZ_00000505">
        <obo:RO_0001025 rdf:resource="http://purl.obolibrary.org/obo/GAZ_00000499"/>
        <oboInOwl:hasOBONamespace>GAZ</oboInOwl:hasOBONamespace>
        <oboInOwl:id>GAZ:00000505</oboInOwl:id>
        <rdfs:label>Tencal Mita</rdfs:label>
    </owl:NamedIndividual>
    


    <!-- http://purl.obolibrary.org/obo/GAZ_00000506 -->

    <owl:NamedIndividual rdf:about="http://purl.obolibrary.org/obo/GAZ_00000506">
        <obo:RO_0001025 rdf:resource="http://purl.obolibrary.org/obo/GAZ_00000499"/>
        <obo:IAO_0000115>A populated place.</obo:IAO_0000115>
        <oboInOwl:hasOBONamespace>GAZ</oboInOwl:hasOBONamespace>
        <oboInOwl:id>GAZ:00000506</oboInOwl:id>
        <rdfs:label>El Barrial</rdfs:label>
    </owl:NamedIndividual>
    


    <!-- http://purl.obolibrary.org/obo/GAZ_00000507 -->

    <owl:NamedIndividual rdf:about="http://purl.obolibrary.org/obo/GAZ_00000507">
        <obo:RO_0001025 rdf:resource="http://purl.obolibrary.org/obo/GAZ_00000499"/>
        <obo:IAO_0000115>A crater lake.</obo:IAO_0000115>
        <oboInOwl:hasOBONamespace>GAZ</oboInOwl:hasOBONamespace>
        <oboInOwl:id>GAZ:00000507</oboInOwl:id>
        <rdfs:label>Laguna de Retana</rdfs:label>
    </owl:NamedIndividual>
    


    <!-- http://purl.obolibrary.org/obo/GAZ_00000508 -->

    <owl:NamedIndividual rdf:about="http://purl.obolibrary.org/obo/GAZ_00000508"/>
    


    <!-- http://purl.obolibrary.org/obo/GAZ_00000509 -->

    <owl:NamedIndividual rdf:about="http://purl.obolibrary.org/obo/GAZ_00000509">
        <rdf:type rdf:resource="http://purl.obolibrary.org/obo/ENVO_00000856"/>
        <obo:RO_0001025 rdf:resource="http://purl.obolibrary.org/obo/GAZ_00000508"/>
        <obo:IAO_0000115>A municipality in the El Peten Department of Guatemala.</obo:IAO_0000115>
        <oboInOwl:hasOBONamespace>GAZ</oboInOwl:hasOBONamespace>
        <oboInOwl:id>GAZ:00000509</oboInOwl:id>
        <rdfs:label>Municipality of Sayaxche</rdfs:label>
    </owl:NamedIndividual>
    


    <!-- http://purl.obolibrary.org/obo/GAZ_00000510 -->

    <owl:NamedIndividual rdf:about="http://purl.obolibrary.org/obo/GAZ_00000510"/>
    


    <!-- http://purl.obolibrary.org/obo/GAZ_00000511 -->

    <owl:NamedIndividual rdf:about="http://purl.obolibrary.org/obo/GAZ_00000511">
        <rdf:type rdf:resource="http://purl.obolibrary.org/obo/ENVO_00000856"/>
        <obo:RO_0001025 rdf:resource="http://purl.obolibrary.org/obo/GAZ_00000510"/>
        <obo:IAO_0000115>A municipality in the Quetzaltenango Department of Guatemala.</obo:IAO_0000115>
        <oboInOwl:hasOBONamespace>GAZ</oboInOwl:hasOBONamespace>
        <oboInOwl:id>GAZ:00000511</oboInOwl:id>
        <rdfs:label>Municipality of Palestina de Los Altos</rdfs:label>
    </owl:NamedIndividual>
    


    <!-- http://purl.obolibrary.org/obo/GAZ_00000512 -->

    <owl:NamedIndividual rdf:about="http://purl.obolibrary.org/obo/GAZ_00000512">
        <obo:RO_0001025 rdf:resource="http://purl.obolibrary.org/obo/GAZ_00000510"/>
        <oboInOwl:hasOBONamespace>GAZ</oboInOwl:hasOBONamespace>
        <oboInOwl:id>GAZ:00000512</oboInOwl:id>
        <rdfs:label>Teneria Europea</rdfs:label>
    </owl:NamedIndividual>
    


    <!-- http://purl.obolibrary.org/obo/GAZ_00000513 -->

    <owl:NamedIndividual rdf:about="http://purl.obolibrary.org/obo/GAZ_00000513">
        <obo:RO_0001025 rdf:resource="http://purl.obolibrary.org/obo/GAZ_00000510"/>
        <oboInOwl:hasOBONamespace>GAZ</oboInOwl:hasOBONamespace>
        <oboInOwl:id>GAZ:00000513</oboInOwl:id>
        <rdfs:label>Bre de Victoria</rdfs:label>
    </owl:NamedIndividual>
    


    <!-- http://purl.obolibrary.org/obo/GAZ_00000514 -->

    <owl:NamedIndividual rdf:about="http://purl.obolibrary.org/obo/GAZ_00000514">
        <obo:RO_0001025 rdf:resource="http://purl.obolibrary.org/obo/GAZ_00000510"/>
        <oboInOwl:hasOBONamespace>GAZ</oboInOwl:hasOBONamespace>
        <oboInOwl:id>GAZ:00000514</oboInOwl:id>
        <rdfs:label>Labor San Jose</rdfs:label>
    </owl:NamedIndividual>
    


    <!-- http://purl.obolibrary.org/obo/GAZ_00000515 -->

    <owl:NamedIndividual rdf:about="http://purl.obolibrary.org/obo/GAZ_00000515">
        <obo:RO_0001025 rdf:resource="http://purl.obolibrary.org/obo/GAZ_00000510"/>
        <obo:IAO_0000115>A populated place.</obo:IAO_0000115>
        <oboInOwl:hasOBONamespace>GAZ</oboInOwl:hasOBONamespace>
        <oboInOwl:id>GAZ:00000515</oboInOwl:id>
        <rdfs:label>La Democracia</rdfs:label>
    </owl:NamedIndividual>
    


    <!-- http://purl.obolibrary.org/obo/GAZ_00000516 -->

    <owl:NamedIndividual rdf:about="http://purl.obolibrary.org/obo/GAZ_00000516">
        <obo:RO_0001025 rdf:resource="http://purl.obolibrary.org/obo/GAZ_00000510"/>
        <oboInOwl:hasOBONamespace>GAZ</oboInOwl:hasOBONamespace>
        <oboInOwl:id>GAZ:00000516</oboInOwl:id>
        <rdfs:label>Chiquiral</rdfs:label>
    </owl:NamedIndividual>
    


    <!-- http://purl.obolibrary.org/obo/GAZ_00000517 -->

    <owl:NamedIndividual rdf:about="http://purl.obolibrary.org/obo/GAZ_00000517"/>
    


    <!-- http://purl.obolibrary.org/obo/GAZ_00000518 -->

    <owl:NamedIndividual rdf:about="http://purl.obolibrary.org/obo/GAZ_00000518">
        <rdf:type rdf:resource="http://purl.obolibrary.org/obo/ENVO_00000856"/>
        <obo:RO_0001025 rdf:resource="http://purl.obolibrary.org/obo/GAZ_00000517"/>
        <obo:IAO_0000115>A municipality in the Guatemalan Department of El Quiche.</obo:IAO_0000115>
        <oboInOwl:hasOBONamespace>GAZ</oboInOwl:hasOBONamespace>
        <oboInOwl:id>GAZ:00000518</oboInOwl:id>
        <rdfs:label>Municipality of San Gaspar Chajul</rdfs:label>
    </owl:NamedIndividual>
    


    <!-- http://purl.obolibrary.org/obo/GAZ_00000519 -->

    <owl:NamedIndividual rdf:about="http://purl.obolibrary.org/obo/GAZ_00000519">
        <rdf:type rdf:resource="http://purl.obolibrary.org/obo/ENVO_00000856"/>
        <obo:RO_0001025 rdf:resource="http://purl.obolibrary.org/obo/GAZ_00000517"/>
        <obo:IAO_0000115>A municipality in the Guatemalan Department of El Quiche.</obo:IAO_0000115>
        <oboInOwl:hasOBONamespace>GAZ</oboInOwl:hasOBONamespace>
        <oboInOwl:id>GAZ:00000519</oboInOwl:id>
        <rdfs:label>Municipality of Santa Maria Nebaj</rdfs:label>
    </owl:NamedIndividual>
    


    <!-- http://purl.obolibrary.org/obo/GAZ_00000520 -->

    <owl:NamedIndividual rdf:about="http://purl.obolibrary.org/obo/GAZ_00000520">
        <rdf:type rdf:resource="http://purl.obolibrary.org/obo/ENVO_00000856"/>
        <obo:RO_0001025 rdf:resource="http://purl.obolibrary.org/obo/GAZ_00000517"/>
        <obo:IAO_0000115>A municipality in the Guatemalan Department of El Quiche.</obo:IAO_0000115>
        <oboInOwl:hasOBONamespace>GAZ</oboInOwl:hasOBONamespace>
        <oboInOwl:id>GAZ:00000520</oboInOwl:id>
        <rdfs:label>Municipality of Uspantan</rdfs:label>
    </owl:NamedIndividual>
    


    <!-- http://purl.obolibrary.org/obo/GAZ_00000521 -->

    <owl:NamedIndividual rdf:about="http://purl.obolibrary.org/obo/GAZ_00000521">
        <obo:RO_0001025 rdf:resource="http://purl.obolibrary.org/obo/GAZ_00000517"/>
        <obo:IAO_0000115>A locality.</obo:IAO_0000115>
        <oboInOwl:hasOBONamespace>GAZ</oboInOwl:hasOBONamespace>
        <oboInOwl:id>GAZ:00000521</oboInOwl:id>
        <rdfs:label>Santa Gertrudis</rdfs:label>
    </owl:NamedIndividual>
    


    <!-- http://purl.obolibrary.org/obo/GAZ_00000522 -->

    <owl:NamedIndividual rdf:about="http://purl.obolibrary.org/obo/GAZ_00000522"/>
    


    <!-- http://purl.obolibrary.org/obo/GAZ_00000523 -->

    <owl:NamedIndividual rdf:about="http://purl.obolibrary.org/obo/GAZ_00000523">
        <rdf:type rdf:resource="http://purl.obolibrary.org/obo/ENVO_00000856"/>
        <obo:RO_0001025 rdf:resource="http://purl.obolibrary.org/obo/GAZ_00000522"/>
        <obo:IAO_0000115>A municipality in the Retalhuleu Department in southwestern Guatemala.</obo:IAO_0000115>
        <oboInOwl:hasOBONamespace>GAZ</oboInOwl:hasOBONamespace>
        <oboInOwl:id>GAZ:00000523</oboInOwl:id>
        <rdfs:label>Municipality of El Asintal</rdfs:label>
    </owl:NamedIndividual>
    


    <!-- http://purl.obolibrary.org/obo/GAZ_00000524 -->

    <owl:NamedIndividual rdf:about="http://purl.obolibrary.org/obo/GAZ_00000524">
        <obo:RO_0001025 rdf:resource="http://purl.obolibrary.org/obo/GAZ_00000522"/>
        <oboInOwl:hasOBONamespace>GAZ</oboInOwl:hasOBONamespace>
        <oboInOwl:id>GAZ:00000524</oboInOwl:id>
        <rdfs:label>Canton Recuerdo</rdfs:label>
    </owl:NamedIndividual>
    


    <!-- http://purl.obolibrary.org/obo/GAZ_00000525 -->

    <owl:NamedIndividual rdf:about="http://purl.obolibrary.org/obo/GAZ_00000525"/>
    


    <!-- http://purl.obolibrary.org/obo/GAZ_00000526 -->

    <owl:NamedIndividual rdf:about="http://purl.obolibrary.org/obo/GAZ_00000526">
        <rdf:type rdf:resource="http://purl.obolibrary.org/obo/ENVO_00000856"/>
        <obo:RO_0001025 rdf:resource="http://purl.obolibrary.org/obo/GAZ_00000525"/>
        <obo:IAO_0000115>A municipality in the Guatemalan Department of Sacatepequez.</obo:IAO_0000115>
        <oboInOwl:hasOBONamespace>GAZ</oboInOwl:hasOBONamespace>
        <oboInOwl:id>GAZ:00000526</oboInOwl:id>
        <rdfs:label>Municipality of Alotenango</rdfs:label>
    </owl:NamedIndividual>
    


    <!-- http://purl.obolibrary.org/obo/GAZ_00000527 -->

    <owl:NamedIndividual rdf:about="http://purl.obolibrary.org/obo/GAZ_00000527">
        <obo:RO_0001025 rdf:resource="http://purl.obolibrary.org/obo/GAZ_00000545"/>
        <obo:IAO_0000115>A populated place.</obo:IAO_0000115>
        <oboInOwl:hasOBONamespace>GAZ</oboInOwl:hasOBONamespace>
        <oboInOwl:id>GAZ:00000527</oboInOwl:id>
        <rdfs:label>Las Chapinas</rdfs:label>
    </owl:NamedIndividual>
    


    <!-- http://purl.obolibrary.org/obo/GAZ_00000528 -->

    <owl:NamedIndividual rdf:about="http://purl.obolibrary.org/obo/GAZ_00000528">
        <obo:RO_0001025 rdf:resource="http://purl.obolibrary.org/obo/GAZ_00000525"/>
        <oboInOwl:hasOBONamespace>GAZ</oboInOwl:hasOBONamespace>
        <oboInOwl:id>GAZ:00000528</oboInOwl:id>
        <rdfs:label>Finca La Union</rdfs:label>
    </owl:NamedIndividual>
    


    <!-- http://purl.obolibrary.org/obo/GAZ_00000529 -->

    <owl:NamedIndividual rdf:about="http://purl.obolibrary.org/obo/GAZ_00000529"/>
    


    <!-- http://purl.obolibrary.org/obo/GAZ_00000530 -->

    <owl:NamedIndividual rdf:about="http://purl.obolibrary.org/obo/GAZ_00000530">
        <rdf:type rdf:resource="http://purl.obolibrary.org/obo/ENVO_00000856"/>
        <obo:RO_0001025 rdf:resource="http://purl.obolibrary.org/obo/GAZ_00000529"/>
        <obo:IAO_0000115>A municipality in the San Marcos Department of Guatemala.</obo:IAO_0000115>
        <oboInOwl:hasOBONamespace>GAZ</oboInOwl:hasOBONamespace>
        <oboInOwl:id>GAZ:00000530</oboInOwl:id>
        <rdfs:label>Municipality of Comitancillo</rdfs:label>
    </owl:NamedIndividual>
    


    <!-- http://purl.obolibrary.org/obo/GAZ_00000531 -->

    <owl:NamedIndividual rdf:about="http://purl.obolibrary.org/obo/GAZ_00000531">
        <rdf:type rdf:resource="http://purl.obolibrary.org/obo/ENVO_00000856"/>
        <obo:RO_0001025 rdf:resource="http://purl.obolibrary.org/obo/GAZ_00000529"/>
        <obo:IAO_0000115>A municipality in the San Marcos Department of Guatemala.</obo:IAO_0000115>
        <oboInOwl:hasOBONamespace>GAZ</oboInOwl:hasOBONamespace>
        <oboInOwl:id>GAZ:00000531</oboInOwl:id>
        <rdfs:label>Municipality of Esquipulas Palo Gordo</rdfs:label>
    </owl:NamedIndividual>
    


    <!-- http://purl.obolibrary.org/obo/GAZ_00000532 -->

    <owl:NamedIndividual rdf:about="http://purl.obolibrary.org/obo/GAZ_00000532">
        <rdf:type rdf:resource="http://purl.obolibrary.org/obo/ENVO_00000856"/>
        <obo:RO_0001025 rdf:resource="http://purl.obolibrary.org/obo/GAZ_00000529"/>
        <obo:IAO_0000115>A municipality in the San Marcos Department of Guatemala.</obo:IAO_0000115>
        <oboInOwl:hasOBONamespace>GAZ</oboInOwl:hasOBONamespace>
        <oboInOwl:id>GAZ:00000532</oboInOwl:id>
        <rdfs:label>Municipality of Tejutla</rdfs:label>
    </owl:NamedIndividual>
    


    <!-- http://purl.obolibrary.org/obo/GAZ_00000533 -->

    <owl:NamedIndividual rdf:about="http://purl.obolibrary.org/obo/GAZ_00000533">
        <obo:RO_0001025 rdf:resource="http://purl.obolibrary.org/obo/GAZ_00000532"/>
        <oboInOwl:hasOBONamespace>GAZ</oboInOwl:hasOBONamespace>
        <oboInOwl:id>GAZ:00000533</oboInOwl:id>
        <rdfs:label>Pulas</rdfs:label>
    </owl:NamedIndividual>
    


    <!-- http://purl.obolibrary.org/obo/GAZ_00000534 -->

    <owl:NamedIndividual rdf:about="http://purl.obolibrary.org/obo/GAZ_00000534">
        <rdf:type rdf:resource="http://purl.obolibrary.org/obo/ENVO_00000856"/>
        <obo:RO_0001025 rdf:resource="http://purl.obolibrary.org/obo/GAZ_00000529"/>
        <obo:IAO_0000115>A municipality in the San Marcos Department of Guatemala.</obo:IAO_0000115>
        <oboInOwl:hasOBONamespace>GAZ</oboInOwl:hasOBONamespace>
        <oboInOwl:id>GAZ:00000534</oboInOwl:id>
        <rdfs:label>Municipality of San Pedro Sacatepequez</rdfs:label>
    </owl:NamedIndividual>
    


    <!-- http://purl.obolibrary.org/obo/GAZ_00000535 -->

    <owl:NamedIndividual rdf:about="http://purl.obolibrary.org/obo/GAZ_00000535">
        <obo:RO_0001025 rdf:resource="http://purl.obolibrary.org/obo/GAZ_00000529"/>
        <obo:IAO_0000115>A populated place.</obo:IAO_0000115>
        <oboInOwl:hasOBONamespace>GAZ</oboInOwl:hasOBONamespace>
        <oboInOwl:id>GAZ:00000535</oboInOwl:id>
        <rdfs:label>La Grandeza</rdfs:label>
    </owl:NamedIndividual>
    


    <!-- http://purl.obolibrary.org/obo/GAZ_00000536 -->

    <owl:NamedIndividual rdf:about="http://purl.obolibrary.org/obo/GAZ_00000536">
        <obo:RO_0001025 rdf:resource="http://purl.obolibrary.org/obo/GAZ_00000529"/>
        <obo:IAO_0000115>A populated place.</obo:IAO_0000115>
        <oboInOwl:hasOBONamespace>GAZ</oboInOwl:hasOBONamespace>
        <oboInOwl:id>GAZ:00000536</oboInOwl:id>
        <rdfs:label>Las Lagunas</rdfs:label>
    </owl:NamedIndividual>
    


    <!-- http://purl.obolibrary.org/obo/GAZ_00000537 -->

    <owl:NamedIndividual rdf:about="http://purl.obolibrary.org/obo/GAZ_00000537">
        <obo:RO_0001025 rdf:resource="http://purl.obolibrary.org/obo/GAZ_00000529"/>
        <oboInOwl:hasOBONamespace>GAZ</oboInOwl:hasOBONamespace>
        <oboInOwl:id>GAZ:00000537</oboInOwl:id>
        <rdfs:label>Entre Rios</rdfs:label>
    </owl:NamedIndividual>
    


    <!-- http://purl.obolibrary.org/obo/GAZ_00000538 -->

    <owl:NamedIndividual rdf:about="http://purl.obolibrary.org/obo/GAZ_00000538">
        <obo:RO_0001025 rdf:resource="http://purl.obolibrary.org/obo/GAZ_00000529"/>
        <obo:IAO_0000115>A populated place.</obo:IAO_0000115>
        <oboInOwl:hasOBONamespace>GAZ</oboInOwl:hasOBONamespace>
        <oboInOwl:id>GAZ:00000538</oboInOwl:id>
        <rdfs:label>Serchil</rdfs:label>
    </owl:NamedIndividual>
    


    <!-- http://purl.obolibrary.org/obo/GAZ_00000539 -->

    <owl:NamedIndividual rdf:about="http://purl.obolibrary.org/obo/GAZ_00000539">
        <obo:RO_0001025 rdf:resource="http://purl.obolibrary.org/obo/GAZ_00000529"/>
        <obo:IAO_0000115>A populated place.</obo:IAO_0000115>
        <oboInOwl:hasOBONamespace>GAZ</oboInOwl:hasOBONamespace>
        <oboInOwl:id>GAZ:00000539</oboInOwl:id>
        <rdfs:label>Tuichilupe</rdfs:label>
    </owl:NamedIndividual>
    


    <!-- http://purl.obolibrary.org/obo/GAZ_00000540 -->

    <owl:NamedIndividual rdf:about="http://purl.obolibrary.org/obo/GAZ_00000540"/>
    


    <!-- http://purl.obolibrary.org/obo/GAZ_00000541 -->

    <owl:NamedIndividual rdf:about="http://purl.obolibrary.org/obo/GAZ_00000541"/>
    


    <!-- http://purl.obolibrary.org/obo/GAZ_00000542 -->

    <owl:NamedIndividual rdf:about="http://purl.obolibrary.org/obo/GAZ_00000542">
        <obo:RO_0001025 rdf:resource="http://purl.obolibrary.org/obo/GAZ_00056113"/>
        <obo:IAO_0000115>A relatively small, private center dedicated to the promotion of local Mayan culture. It holds the most extensive teaching medicinal plant garden in the Lake Atitlan Basin.</obo:IAO_0000115>
        <oboInOwl:hasOBONamespace>GAZ</oboInOwl:hasOBONamespace>
        <oboInOwl:id>GAZ:00000542</oboInOwl:id>
        <rdfs:label>Centro Cultural Los Encuentros</rdfs:label>
    </owl:NamedIndividual>
    


    <!-- http://purl.obolibrary.org/obo/GAZ_00000543 -->

    <owl:NamedIndividual rdf:about="http://purl.obolibrary.org/obo/GAZ_00000543">
        <obo:RO_0001025 rdf:resource="http://purl.obolibrary.org/obo/GAZ_00000541"/>
        <oboInOwl:hasOBONamespace>GAZ</oboInOwl:hasOBONamespace>
        <oboInOwl:id>GAZ:00000543</oboInOwl:id>
        <rdfs:label>Codines</rdfs:label>
    </owl:NamedIndividual>
    


    <!-- http://purl.obolibrary.org/obo/GAZ_00000544 -->

    <owl:NamedIndividual rdf:about="http://purl.obolibrary.org/obo/GAZ_00000544">
        <obo:RO_0001025 rdf:resource="http://purl.obolibrary.org/obo/GAZ_00000541"/>
        <oboInOwl:hasOBONamespace>GAZ</oboInOwl:hasOBONamespace>
        <oboInOwl:id>GAZ:00000544</oboInOwl:id>
        <rdfs:label>Catxac</rdfs:label>
    </owl:NamedIndividual>
    


    <!-- http://purl.obolibrary.org/obo/GAZ_00000545 -->

    <owl:NamedIndividual rdf:about="http://purl.obolibrary.org/obo/GAZ_00000545"/>
    


    <!-- http://purl.obolibrary.org/obo/GAZ_00000546 -->

    <owl:NamedIndividual rdf:about="http://purl.obolibrary.org/obo/GAZ_00000546">
        <rdf:type rdf:resource="http://purl.obolibrary.org/obo/ENVO_00000856"/>
        <obo:RO_0001025 rdf:resource="http://purl.obolibrary.org/obo/GAZ_00000545"/>
        <obo:IAO_0000115>A municipality in the Suchitepequez Department of Guatemala.</obo:IAO_0000115>
        <oboInOwl:hasOBONamespace>GAZ</oboInOwl:hasOBONamespace>
        <oboInOwl:id>GAZ:00000546</oboInOwl:id>
        <rdfs:label>Municipality of San Antonio Suchitepequez</rdfs:label>
    </owl:NamedIndividual>
    


    <!-- http://purl.obolibrary.org/obo/GAZ_00000547 -->

    <owl:NamedIndividual rdf:about="http://purl.obolibrary.org/obo/GAZ_00000547">
        <obo:RO_0001025 rdf:resource="http://purl.obolibrary.org/obo/GAZ_00000545"/>
        <oboInOwl:hasOBONamespace>GAZ</oboInOwl:hasOBONamespace>
        <oboInOwl:id>GAZ:00000547</oboInOwl:id>
        <rdfs:label>Montecristo</rdfs:label>
    </owl:NamedIndividual>
    


    <!-- http://purl.obolibrary.org/obo/GAZ_00000548 -->

    <owl:NamedIndividual rdf:about="http://purl.obolibrary.org/obo/GAZ_00000548"/>
    


    <!-- http://purl.obolibrary.org/obo/GAZ_00000549 -->

    <owl:NamedIndividual rdf:about="http://purl.obolibrary.org/obo/GAZ_00000549"/>
    


    <!-- http://purl.obolibrary.org/obo/GAZ_00000550 -->

    <owl:NamedIndividual rdf:about="http://purl.obolibrary.org/obo/GAZ_00000550">
        <obo:RO_0001025 rdf:resource="http://purl.obolibrary.org/obo/GAZ_00000549"/>
        <oboInOwl:hasOBONamespace>GAZ</oboInOwl:hasOBONamespace>
        <oboInOwl:id>GAZ:00000550</oboInOwl:id>
        <rdfs:label>Pacoc</rdfs:label>
    </owl:NamedIndividual>
    


    <!-- http://purl.obolibrary.org/obo/GAZ_00000551 -->

    <owl:NamedIndividual rdf:about="http://purl.obolibrary.org/obo/GAZ_00000551">
        <obo:RO_0001025 rdf:resource="http://purl.obolibrary.org/obo/GAZ_00000549"/>
        <obo:IAO_0000115>A locality.</obo:IAO_0000115>
        <oboInOwl:hasOBONamespace>GAZ</oboInOwl:hasOBONamespace>
        <oboInOwl:id>GAZ:00000551</oboInOwl:id>
        <rdfs:label>Tierra Blanca</rdfs:label>
    </owl:NamedIndividual>
    


    <!-- http://purl.obolibrary.org/obo/GAZ_00000552 -->

    <owl:NamedIndividual rdf:about="http://purl.obolibrary.org/obo/GAZ_00000552">
        <obo:RO_0001025 rdf:resource="http://purl.obolibrary.org/obo/GAZ_00000549"/>
        <obo:IAO_0000115>A populated place.</obo:IAO_0000115>
        <oboInOwl:hasOBONamespace>GAZ</oboInOwl:hasOBONamespace>
        <oboInOwl:id>GAZ:00000552</oboInOwl:id>
        <rdfs:label>Candelaria</rdfs:label>
    </owl:NamedIndividual>
    


    <!-- http://purl.obolibrary.org/obo/GAZ_00000856 -->

    <owl:NamedIndividual rdf:about="http://purl.obolibrary.org/obo/GAZ_00000856">
        <obo:RO_0001025 rdf:resource="http://purl.obolibrary.org/obo/GAZ_00000548"/>
        <obo:IAO_0000115>A populated place.</obo:IAO_0000115>
        <oboInOwl:hasOBONamespace>GAZ</oboInOwl:hasOBONamespace>
        <oboInOwl:id>GAZ:00000856</oboInOwl:id>
        <rdfs:label>Pie de La Cuesta</rdfs:label>
    </owl:NamedIndividual>
    


    <!-- http://purl.obolibrary.org/obo/GAZ_00000873 -->

    <owl:NamedIndividual rdf:about="http://purl.obolibrary.org/obo/GAZ_00000873">
        <obo:RO_0001025 rdf:resource="http://purl.obolibrary.org/obo/GAZ_00002936"/>
        <oboInOwl:hasOBONamespace>GAZ</oboInOwl:hasOBONamespace>
        <oboInOwl:id>GAZ:00000873</oboInOwl:id>
        <rdfs:label>Barrio Garibaldi</rdfs:label>
    </owl:NamedIndividual>
    


    <!-- http://purl.obolibrary.org/obo/GAZ_00000874 -->

    <owl:NamedIndividual rdf:about="http://purl.obolibrary.org/obo/GAZ_00000874">
        <obo:RO_0001025 rdf:resource="http://purl.obolibrary.org/obo/GAZ_00002936"/>
        <oboInOwl:hasOBONamespace>GAZ</oboInOwl:hasOBONamespace>
        <oboInOwl:id>GAZ:00000874</oboInOwl:id>
        <rdfs:label>Calzad A Benito Juar</rdfs:label>
    </owl:NamedIndividual>
    


    <!-- http://purl.obolibrary.org/obo/GAZ_00000875 -->

    <owl:NamedIndividual rdf:about="http://purl.obolibrary.org/obo/GAZ_00000875">
        <obo:RO_0001025 rdf:resource="http://purl.obolibrary.org/obo/GAZ_00000439"/>
        <oboInOwl:hasOBONamespace>GAZ</oboInOwl:hasOBONamespace>
        <oboInOwl:id>GAZ:00000875</oboInOwl:id>
        <rdfs:label>Canton Bola de Oro</rdfs:label>
    </owl:NamedIndividual>
    


    <!-- http://purl.obolibrary.org/obo/GAZ_00000876 -->

    <owl:NamedIndividual rdf:about="http://purl.obolibrary.org/obo/GAZ_00000876">
        <obo:RO_0001025 rdf:resource="http://purl.obolibrary.org/obo/GAZ_00002936"/>
        <oboInOwl:hasOBONamespace>GAZ</oboInOwl:hasOBONamespace>
        <oboInOwl:id>GAZ:00000876</oboInOwl:id>
        <rdfs:label>Canton Chalchequin</rdfs:label>
    </owl:NamedIndividual>
    


    <!-- http://purl.obolibrary.org/obo/GAZ_00000878 -->

    <owl:NamedIndividual rdf:about="http://purl.obolibrary.org/obo/GAZ_00000878">
        <rdf:type rdf:resource="http://purl.obolibrary.org/obo/ENVO_00000856"/>
        <obo:RO_0001025 rdf:resource="http://purl.obolibrary.org/obo/GAZ_00000476"/>
        <obo:IAO_0000115>A municipality in the El Progreso Department of Guatemala.</obo:IAO_0000115>
        <oboInOwl:hasOBONamespace>GAZ</oboInOwl:hasOBONamespace>
        <oboInOwl:id>GAZ:00000878</oboInOwl:id>
        <rdfs:label>Municipality of Sanarate</rdfs:label>
    </owl:NamedIndividual>
    


    <!-- http://purl.obolibrary.org/obo/GAZ_00000879 -->

    <owl:NamedIndividual rdf:about="http://purl.obolibrary.org/obo/GAZ_00000879">
        <obo:RO_0001025 rdf:resource="http://purl.obolibrary.org/obo/GAZ_00000878"/>
        <oboInOwl:hasOBONamespace>GAZ</oboInOwl:hasOBONamespace>
        <oboInOwl:id>GAZ:00000879</oboInOwl:id>
        <rdfs:label>La Cumbre</rdfs:label>
    </owl:NamedIndividual>
    


    <!-- http://purl.obolibrary.org/obo/GAZ_00000880 -->

    <owl:NamedIndividual rdf:about="http://purl.obolibrary.org/obo/GAZ_00000880">
        <obo:RO_0001025 rdf:resource="http://purl.obolibrary.org/obo/GAZ_00002936"/>
        <oboInOwl:hasOBONamespace>GAZ</oboInOwl:hasOBONamespace>
        <oboInOwl:id>GAZ:00000880</oboInOwl:id>
        <rdfs:label>La Vuelta de Los Ram</rdfs:label>
    </owl:NamedIndividual>
    


    <!-- http://purl.obolibrary.org/obo/GAZ_00000881 -->

    <owl:NamedIndividual rdf:about="http://purl.obolibrary.org/obo/GAZ_00000881">
        <rdf:type rdf:resource="http://purl.obolibrary.org/obo/ENVO_00000856"/>
        <obo:RO_0001025 rdf:resource="http://purl.obolibrary.org/obo/GAZ_00000517"/>
        <obo:IAO_0000115>A municipality in the Guatemalan Department of El Quiche.</obo:IAO_0000115>
        <oboInOwl:hasOBONamespace>GAZ</oboInOwl:hasOBONamespace>
        <oboInOwl:id>GAZ:00000881</oboInOwl:id>
        <rdfs:label>Municipality of San Pedro Jocopilas</rdfs:label>
    </owl:NamedIndividual>
    


    <!-- http://purl.obolibrary.org/obo/GAZ_00002936 -->

    <owl:NamedIndividual rdf:about="http://purl.obolibrary.org/obo/GAZ_00002936">
        <rdf:type rdf:resource="http://purl.obolibrary.org/obo/ENVO_00000009"/>
        <obo:IAO_0000115>A country in Central America bordered by Mexico to the northwest, the Pacific Ocean to the southwest, Belize and the Caribbean Sea to the northeast, and Honduras and El Salvador to the southeast. Guatemala is divided into 22 departments (departamentos) and sub-divided into about 332 municipalities (municipios).</obo:IAO_0000115>
        <oboInOwl:hasOBONamespace>GAZ</oboInOwl:hasOBONamespace>
        <oboInOwl:id>GAZ:00002936</oboInOwl:id>
        <rdfs:label>Guatemala</rdfs:label>
    </owl:NamedIndividual>
    


    <!-- http://purl.obolibrary.org/obo/GAZ_00005152 -->

    <owl:NamedIndividual rdf:about="http://purl.obolibrary.org/obo/GAZ_00005152">
        <obo:RO_0001025 rdf:resource="http://purl.obolibrary.org/obo/GAZ_00002936"/>
    </owl:NamedIndividual>
    


    <!-- http://purl.obolibrary.org/obo/GAZ_00005153 -->

    <owl:NamedIndividual rdf:about="http://purl.obolibrary.org/obo/GAZ_00005153">
        <obo:RO_0001025 rdf:resource="http://purl.obolibrary.org/obo/GAZ_00002936"/>
    </owl:NamedIndividual>
    


    <!-- http://purl.obolibrary.org/obo/GAZ_00005154 -->

    <owl:NamedIndividual rdf:about="http://purl.obolibrary.org/obo/GAZ_00005154">
        <obo:RO_0001025 rdf:resource="http://purl.obolibrary.org/obo/GAZ_00005155"/>
    </owl:NamedIndividual>
    


    <!-- http://purl.obolibrary.org/obo/GAZ_00005155 -->

    <owl:NamedIndividual rdf:about="http://purl.obolibrary.org/obo/GAZ_00005155"/>
    


    <!-- http://purl.obolibrary.org/obo/GAZ_00007985 -->

    <owl:NamedIndividual rdf:about="http://purl.obolibrary.org/obo/GAZ_00007985">
        <obo:RO_0001025 rdf:resource="http://purl.obolibrary.org/obo/GAZ_00248547"/>
        <obo:IAO_0000115>An airport.</obo:IAO_0000115>
        <oboInOwl:hasOBONamespace>GAZ</oboInOwl:hasOBONamespace>
        <oboInOwl:id>GAZ:00007985</oboInOwl:id>
        <rdfs:label>La Aurora International Airport</rdfs:label>
    </owl:NamedIndividual>
    


    <!-- http://purl.obolibrary.org/obo/GAZ_00056095 -->

    <owl:NamedIndividual rdf:about="http://purl.obolibrary.org/obo/GAZ_00056095">
        <obo:RO_0001025 rdf:resource="http://purl.obolibrary.org/obo/GAZ_00000529"/>
        <obo:IAO_0000115>A 4060 m high composite stratovolcano that straddles the Mexico/Guatemala border at the NW end of the Central American volcanic belt. The volcano rises 1800 m above deeply dissected plutonic and metamorphic terrain. Three large calderas breached to the south, and the elongated summit region is dominated by a series of lava domes intruded along a NE-SW trend. Volcanism has migrated to the SW, and a small adventive lava dome is located in the crater of the youngest volcano, San Antonio, on the upper SW flank. Viscous lava flow complexes are found on the north and south flanks, and lobate lahar deposits fill many valleys. Radial drainages on the Guatemalan side are deflected by surrounding mountains into the Pacific coastal plain on the SW side of the volcano. Historical activity at Tacana has been restricted to mild phreatic eruptions, but more powerful explosive activity, including the production of pyroclastic flows, has occurred as recently as about 1950 years ago.</obo:IAO_0000115>
        <oboInOwl:hasOBONamespace>GAZ</oboInOwl:hasOBONamespace>
        <oboInOwl:id>GAZ:00056095</oboInOwl:id>
        <rdfs:label>Volcan Tacana</rdfs:label>
    </owl:NamedIndividual>
    


    <!-- http://purl.obolibrary.org/obo/GAZ_00056097 -->

    <owl:NamedIndividual rdf:about="http://purl.obolibrary.org/obo/GAZ_00056097">
        <rdf:type rdf:resource="http://purl.obolibrary.org/obo/ENVO_00000095"/>
        <obo:RO_0001025 rdf:resource="http://purl.obolibrary.org/obo/GAZ_00000529"/>
        <obo:IAO_0000115>A volcano with two summits, one with a 50-70 m wide crater, that lies along a NW-SE line. A lava flow from the 4220 m high NW summit traveled down a deep valley on the NW flank. The andesitic-dacitic volcano was constructed over the NW end of a large arcuate SW-facing escarpment of uncertain origin.</obo:IAO_0000115>
        <oboInOwl:hasOBONamespace>GAZ</oboInOwl:hasOBONamespace>
        <oboInOwl:id>GAZ:00056097</oboInOwl:id>
        <rdfs:label>Volcan Tajumulco</rdfs:label>
    </owl:NamedIndividual>
    


    <!-- http://purl.obolibrary.org/obo/GAZ_00056098 -->

    <owl:NamedIndividual rdf:about="http://purl.obolibrary.org/obo/GAZ_00056098">
        <obo:RO_0001025 rdf:resource="http://purl.obolibrary.org/obo/GAZ_00000510"/>
        <obo:IAO_0000115>A stratovolcano tahtis one of the most prominent of a chain of large stratovolcanoes that rises dramatically above the Pacific coastal plain of Guatemala. The 3772 m high stratovolcano has a sharp-topped, conical profile that is cut on the SW flank by a large, 1.5 km wide crater. The oval-shaped crater extends from just below the summit of Volcan Santa Maria to the lower flank and was formed during a catastrophic eruption in 1902. The renowned plinian eruption of 1902 that devastated much of SW Guatemala followed a long repose period after construction of the large basaltic-andesite stratovolcano. The massive dacitic Santiaguito lava-dome complex has been growing at the base of the 1902 crater since 1922. Compound dome growth at Santiaguito has occurred episodically from four westward-younging vents, the most recent of which is Caliente. Dome growth has been accompanied by almost continuous minor explosions, with periodic lava extrusion, larger explosions, pyroclastic flows, and lahars.</obo:IAO_0000115>
        <oboInOwl:hasOBONamespace>GAZ</oboInOwl:hasOBONamespace>
        <oboInOwl:id>GAZ:00056098</oboInOwl:id>
        <rdfs:label>Volcan Santa Maria</rdfs:label>
    </owl:NamedIndividual>
    


    <!-- http://purl.obolibrary.org/obo/GAZ_00056099 -->

    <owl:NamedIndividual rdf:about="http://purl.obolibrary.org/obo/GAZ_00056099">
        <obo:RO_0001025 rdf:resource="http://purl.obolibrary.org/obo/GAZ_00056098"/>
        <obo:IAO_0000115>A new volcanic vent formed in 1922 in the enormous crater of Santa Maria, and formed a new volcano. Santiaguito has been erupting ever since and now forms a cone a few hundred m tall, reaching an elevation of about 2,500 m.</obo:IAO_0000115>
        <oboInOwl:hasOBONamespace>GAZ</oboInOwl:hasOBONamespace>
        <oboInOwl:id>GAZ:00056099</oboInOwl:id>
        <rdfs:label>Santiaguito</rdfs:label>
    </owl:NamedIndividual>
    


    <!-- http://purl.obolibrary.org/obo/GAZ_00056100 -->

    <owl:NamedIndividual rdf:about="http://purl.obolibrary.org/obo/GAZ_00056100">
        <obo:IAO_0000115>A mountain range which runs northwest-southeast from the State of Chiapas in Mexico across Guatemala and into El Salvador and Honduras. Most of the volcanoes of Guatemala are a part of this range. A narrow coastal plain lies south the range, between the Sierra Madre and the Pacific Ocean. To the north lie a series of highlands and depressions, including the Chiapas Depression, which separates the Sierra Madre from the Chiapas Plateau, the Guatemalan Highlands, and Honduras&apos; interior highlands. The Sierra forms the main watershed between the Pacific and Atlantic river systems.</obo:IAO_0000115>
        <oboInOwl:hasOBONamespace>GAZ</oboInOwl:hasOBONamespace>
        <oboInOwl:id>GAZ:00056100</oboInOwl:id>
        <rdfs:label>Sierra Madre de Chiapas</rdfs:label>
    </owl:NamedIndividual>
    


    <!-- http://purl.obolibrary.org/obo/GAZ_00056101 -->

    <owl:NamedIndividual rdf:about="http://purl.obolibrary.org/obo/GAZ_00056101">
        <obo:RO_0001025 rdf:resource="http://purl.obolibrary.org/obo/GAZ_00056100"/>
        <obo:IAO_0000115>An andesitic stratovolcano with a 3.3 km wide late-Pleistocene central caldera that is located along the Zunil fault zone. The caldera is surrounded by a ring-dike configuration of dacitic and rhyolitic lava domes. The youngest and only historically active dome complex is Cerro Quemado, located immediately south of Guatemala&apos;s second largest city, Quezaltenango. About 1200 radiocarbon years ago, part of the andesitic-to-dacitic Cerro Quemado dome collapsed, producing a debris avalanche and an associated lateral explosion that swept across the valley to the west as far as the flanks of Siete Orejas volcano. The latest eruption in 1818 produced a blocky 2.5 km-long lava flow. Hot springs are located on the northern and eastern flanks of Cerro Quemado, and the Zunil geothermal field, the site of a geothermal exploration project, lies on the SE flank of Cerro Quemado.</obo:IAO_0000115>
        <oboInOwl:hasOBONamespace>GAZ</oboInOwl:hasOBONamespace>
        <oboInOwl:id>GAZ:00056101</oboInOwl:id>
        <rdfs:label>Almolonga Volcano</rdfs:label>
    </owl:NamedIndividual>
    


    <!-- http://purl.obolibrary.org/obo/GAZ_00056102 -->

    <owl:NamedIndividual rdf:about="http://purl.obolibrary.org/obo/GAZ_00056102">
        <obo:RO_0001025 rdf:resource="http://purl.obolibrary.org/obo/GAZ_00056101"/>
        <obo:IAO_0000115>A volcanic dome.</obo:IAO_0000115>
        <oboInOwl:hasOBONamespace>GAZ</oboInOwl:hasOBONamespace>
        <oboInOwl:id>GAZ:00056102</oboInOwl:id>
        <rdfs:label>Cerro Quemado</rdfs:label>
    </owl:NamedIndividual>
    


    <!-- http://purl.obolibrary.org/obo/GAZ_00056103 -->

    <owl:NamedIndividual rdf:about="http://purl.obolibrary.org/obo/GAZ_00056103">
        <obo:RO_0001025 rdf:resource="http://purl.obolibrary.org/obo/GAZ_00000541"/>
        <obo:IAO_0000115>A large eroded stratovolcano located across a valley SE of Santa Maria volcano. The summit of the volcano is capped by late-Quaternary andesitic tephra. A winding ridge connects Santo Toas to Volcan de Zunil, 4.5 km to the NE, a 3542 m high stratovolcano that forms the topographic high point of the Santo Tomas - Zunil complex. Volcan de Zunil is located on the SW rim of the 4 km wide, 600-m-deep Tzanjuyub caldera, which is breached to the south by the Rio Masa. Several dacitic-rhyolitic lava domes are located on the caldera&apos;s northern flank and the NW flank of Volcan de Zunil. The youngest dome, Cerro Zunil, was last active about 84,000 years ago (K-Ar dating).</obo:IAO_0000115>
        <oboInOwl:hasOBONamespace>GAZ</oboInOwl:hasOBONamespace>
        <oboInOwl:id>GAZ:00056103</oboInOwl:id>
        <rdfs:label>Volcan Santo Tomas</rdfs:label>
    </owl:NamedIndividual>
    


    <!-- http://purl.obolibrary.org/obo/GAZ_00056104 -->

    <owl:NamedIndividual rdf:about="http://purl.obolibrary.org/obo/GAZ_00056104">
        <obo:RO_0001025 rdf:resource="http://purl.obolibrary.org/obo/GAZ_00056103"/>
        <obo:IAO_0000115>A volcanic dome.</obo:IAO_0000115>
        <oboInOwl:hasOBONamespace>GAZ</oboInOwl:hasOBONamespace>
        <oboInOwl:id>GAZ:00056104</oboInOwl:id>
        <rdfs:label>Cerro Zunil</rdfs:label>
    </owl:NamedIndividual>
    


    <!-- http://purl.obolibrary.org/obo/GAZ_00056105 -->

    <owl:NamedIndividual rdf:about="http://purl.obolibrary.org/obo/GAZ_00056105">
        <obo:RO_0001025 rdf:resource="http://purl.obolibrary.org/obo/GAZ_00000541"/>
        <obo:IAO_0000115>One of several prominent conical stratovolcanoes in the Guatemalan highlands. Along with its twin volcano Toliman to the north, it forms a dramatic backdrop to Lake Atitlan, one of the scenic highlights of the country. The 3535 m high summit of Atitlan directly overlies the inferred margin of the Pleistocene Atitlan III caldera and is the highest of three large post-caldera stratovolcanoes constructed near the southern caldera rim. The volcano consequently post-dates the eruption of the voluminous, roughly 85,000-year-old rhyolitic Los Chocoyos tephra associated with formation of the Atitlan III caldera. The historically active andesitic Volcan Atitlan is younger than Toliman, although their earlier activity overlapped. In contrast to Toliman, Atitlan displays a thick pyroclastic cover.</obo:IAO_0000115>
        <oboInOwl:hasOBONamespace>GAZ</oboInOwl:hasOBONamespace>
        <oboInOwl:id>GAZ:00056105</oboInOwl:id>
        <rdfs:label>Volcan Atitlan</rdfs:label>
    </owl:NamedIndividual>
    


    <!-- http://purl.obolibrary.org/obo/GAZ_00056106 -->

    <owl:NamedIndividual rdf:about="http://purl.obolibrary.org/obo/GAZ_00056106">
        <obo:RO_0001025 rdf:resource="http://purl.obolibrary.org/obo/GAZ_00000541"/>
        <obo:IAO_0000115>A large endorheic crater lake in the Guatemalan Highlands. The lake is volcanic in origin, filling an enormous caldera formed in an eruption 84,000 years ago.</obo:IAO_0000115>
        <oboInOwl:hasOBONamespace>GAZ</oboInOwl:hasOBONamespace>
        <oboInOwl:id>GAZ:00056106</oboInOwl:id>
        <rdfs:label>Lago de Atitlan</rdfs:label>
    </owl:NamedIndividual>
    


    <!-- http://purl.obolibrary.org/obo/GAZ_00056107 -->

    <owl:NamedIndividual rdf:about="http://purl.obolibrary.org/obo/GAZ_00056107">
        <obo:RO_0001025 rdf:resource="http://purl.obolibrary.org/obo/GAZ_00068303"/>
        <obo:IAO_0000115>A large andesitic stratovolcano that rises above the south shore of Lake Atitlan. Toliman was constructed within the Pleistocene Atitlan III caldera, near its inferred southern margin. A shallow elliptical crater truncates the summit, and a minor subsidiary peak to the SSW also has a shallow crater. In contrast to the tephra-covered surface of its twin volcano to the south, Volcan Atitlan, the surface of Toliman is draped by prominent thick lava flows. Many of the flows were erupted from vents on the volcano&apos;s flanks and form a highly irregular shoreline on the south side of Lake Atitlan. No historical eruptions are known from Toliman.</obo:IAO_0000115>
        <oboInOwl:hasOBONamespace>GAZ</oboInOwl:hasOBONamespace>
        <oboInOwl:id>GAZ:00056107</oboInOwl:id>
        <rdfs:label>Volcan Toliman</rdfs:label>
    </owl:NamedIndividual>
    


    <!-- http://purl.obolibrary.org/obo/GAZ_00056108 -->

    <owl:NamedIndividual rdf:about="http://purl.obolibrary.org/obo/GAZ_00056108">
        <obo:RO_0001025 rdf:resource="http://purl.obolibrary.org/obo/GAZ_00000525"/>
        <obo:RO_0001025 rdf:resource="http://purl.obolibrary.org/obo/GAZ_00056100"/>
        <obo:IAO_0000115>A stratovolcano that has two principal summits, was constructed during three eruptive periods post-dating the roughly 85,000-year-old Los Chocoyos tephra from Atitlan caldera. An ancestral Acatenango volcano collapsed to the south sometime prior to 43,000 years ago, forming La Democracia debris-avalanche deposit, which covers a wide area of the Pacific coastal plain. Construction of Yepocapa, the northern summit of Acatenango, was completed about 20,000 years ago, after which growth of the southern and highest cone, Pico Central began.</obo:IAO_0000115>
        <oboInOwl:hasOBONamespace>GAZ</oboInOwl:hasOBONamespace>
        <oboInOwl:id>GAZ:00056108</oboInOwl:id>
        <rdfs:label>Volcan de Acatenango</rdfs:label>
    </owl:NamedIndividual>
    


    <!-- http://purl.obolibrary.org/obo/GAZ_00056109 -->

    <owl:NamedIndividual rdf:about="http://purl.obolibrary.org/obo/GAZ_00056109">
        <obo:RO_0001025 rdf:resource="http://purl.obolibrary.org/obo/GAZ_00056108"/>
        <obo:IAO_0000115>A stratovolcano.</obo:IAO_0000115>
        <oboInOwl:hasOBONamespace>GAZ</oboInOwl:hasOBONamespace>
        <oboInOwl:id>GAZ:00056109</oboInOwl:id>
        <rdfs:label>Pico Central</rdfs:label>
    </owl:NamedIndividual>
    


    <!-- http://purl.obolibrary.org/obo/GAZ_00056110 -->

    <owl:NamedIndividual rdf:about="http://purl.obolibrary.org/obo/GAZ_00056110">
        <obo:RO_0001025 rdf:resource="http://purl.obolibrary.org/obo/GAZ_00056108"/>
        <obo:IAO_0000115>The northern summit of Acatenango, a stratovolcano.</obo:IAO_0000115>
        <oboInOwl:hasOBONamespace>GAZ</oboInOwl:hasOBONamespace>
        <oboInOwl:id>GAZ:00056110</oboInOwl:id>
        <rdfs:label>Yepocapa</rdfs:label>
    </owl:NamedIndividual>
    


    <!-- http://purl.obolibrary.org/obo/GAZ_00056111 -->

    <owl:NamedIndividual rdf:about="http://purl.obolibrary.org/obo/GAZ_00056111">
        <obo:RO_0001025 rdf:resource="http://purl.obolibrary.org/obo/GAZ_00000525"/>
        <obo:RO_0001025 rdf:resource="http://purl.obolibrary.org/obo/GAZ_00056100"/>
        <obo:IAO_0000115>A stratovolcano located in Guatemala that has been inactive since the mid 16th century.</obo:IAO_0000115>
        <oboInOwl:hasOBONamespace>GAZ</oboInOwl:hasOBONamespace>
        <oboInOwl:id>GAZ:00056111</oboInOwl:id>
        <rdfs:label>Volcan de Agua</rdfs:label>
    </owl:NamedIndividual>
    


    <!-- http://purl.obolibrary.org/obo/GAZ_00056112 -->

    <owl:NamedIndividual rdf:about="http://purl.obolibrary.org/obo/GAZ_00056112">
        <obo:RO_0001025 rdf:resource="http://purl.obolibrary.org/obo/GAZ_00000439"/>
        <obo:RO_0001025 rdf:resource="http://purl.obolibrary.org/obo/GAZ_00000525"/>
        <obo:IAO_0000115>One of three large stratovolcanoes overlooking Guatemala&apos;s former capital, Antigua. The scarp of an older edifice, Meseta, lies between 3763 m high Fuego and its twin volcano to the north, Acatenango. Construction of Meseta volcano dates back to about 230,000 years and continued until the late Pleistocene or early Holocene. Collapse of Meseta volcano may have produced the massive Escuintla debris-avalanche deposit, which extends about 50 km onto the Pacific coastal plain. Growth of the modern Fuego volcano followed, continuing the southward migration of volcanism that began at Acatenango. In contrast to the mostly andesitic Acatenango volcano, eruptions at Fuego have become more mafic with time, and most historical activity has produced basaltic rocks. Frequent vigorous historical eruptions have been recorded at Fuego since the onset of the Spanish era in 1524, and have produced major ashfalls, along with occasional pyroclastic flows and lava flows.</obo:IAO_0000115>
        <oboInOwl:hasOBONamespace>GAZ</oboInOwl:hasOBONamespace>
        <oboInOwl:id>GAZ:00056112</oboInOwl:id>
        <rdfs:label>Volcan de Fuego</rdfs:label>
    </owl:NamedIndividual>
    


    <!-- http://purl.obolibrary.org/obo/GAZ_00056113 -->

    <owl:NamedIndividual rdf:about="http://purl.obolibrary.org/obo/GAZ_00056113">
        <rdf:type rdf:resource="http://purl.obolibrary.org/obo/ENVO_00000856"/>
        <obo:RO_0001025 rdf:resource="http://purl.obolibrary.org/obo/GAZ_00056114"/>
    </owl:NamedIndividual>
    


    <!-- http://purl.obolibrary.org/obo/GAZ_00056114 -->

    <owl:NamedIndividual rdf:about="http://purl.obolibrary.org/obo/GAZ_00056114">
        <rdf:type rdf:resource="http://purl.obolibrary.org/obo/ENVO_00000856"/>
        <obo:RO_0001025 rdf:resource="http://purl.obolibrary.org/obo/GAZ_00000541"/>
        <obo:IAO_0000115>A municipality in the Solola Department of Guatemala.</obo:IAO_0000115>
        <oboInOwl:hasOBONamespace>GAZ</oboInOwl:hasOBONamespace>
        <oboInOwl:id>GAZ:00056114</oboInOwl:id>
        <rdfs:label>Municipality of Panajachel</rdfs:label>
    </owl:NamedIndividual>
    


    <!-- http://purl.obolibrary.org/obo/GAZ_00056115 -->

    <owl:NamedIndividual rdf:about="http://purl.obolibrary.org/obo/GAZ_00056115">
        <obo:RO_0001025 rdf:resource="http://purl.obolibrary.org/obo/GAZ_00000477"/>
        <obo:IAO_0000115>A complex basaltic volcano constructed just outside the southern topographic rim of the 14 x 16 km Pleistocene Amatitlan caldera. A cluster of dacitic lava domes occupies the southern caldera floor. The post-caldera Pacaya massif includes the Cerro Grande lava dome and a younger volcano to the SW. Collapse of Pacaya volcano about 1100 years ago produced a debris-avalanche deposit that extends 25 km onto the Pacific coastal plain and left an arcuate somma rim inside which the modern Pacaya volcano (MacKenney cone) grew. A subsidiary crater, Cerro Chino, was constructed on the NW somma rim and was last active in the 19th century. During the past several decades, activity at Pacaya has consisted of frequent strombolian eruptions with intermittent lava flow extrusion that has partially filled in the caldera moat and armored the flanks of MacKenney cone, punctuated by occasional larger explosive eruptions that partially destroy the summit of the cone.</obo:IAO_0000115>
        <oboInOwl:hasOBONamespace>GAZ</oboInOwl:hasOBONamespace>
        <oboInOwl:id>GAZ:00056115</oboInOwl:id>
        <rdfs:label>Volcan Pacaya</rdfs:label>
    </owl:NamedIndividual>
    


    <!-- http://purl.obolibrary.org/obo/GAZ_00056116 -->

    <owl:NamedIndividual rdf:about="http://purl.obolibrary.org/obo/GAZ_00056116">
        <obo:RO_0001025 rdf:resource="http://purl.obolibrary.org/obo/GAZ_00000540"/>
        <obo:IAO_0000115>A volcanic field that contains approximately 70 Quaternary cinder cones, generally less than 100 m high. Many of the mostly basaltic cones are located along the strike of the major regional Jalpatagua fault, which extends SE from Guatemala City, north of the chain of stratovolcanoes stretching across Guatemala. The cones were erupted from fracture systems related to the intersection of the Jalpatagua fault with the southern and western margins of the Miocene Santa Rosa de Lima caldera and overlie pyroclastic-flow deposits from Amatitlan caldera to the NW. The age of the most recent eruptions is not known, although the youngest cones post-date the last phase of eruptive activity at Tecuamburro volcano and could be of Holocene age.</obo:IAO_0000115>
        <oboInOwl:hasOBONamespace>GAZ</oboInOwl:hasOBONamespace>
        <oboInOwl:id>GAZ:00056116</oboInOwl:id>
        <rdfs:label>Cuilapa-Barbarena Volcanic Field</rdfs:label>
    </owl:NamedIndividual>
    


    <!-- http://purl.obolibrary.org/obo/GAZ_00056117 -->

    <owl:NamedIndividual rdf:about="http://purl.obolibrary.org/obo/GAZ_00056117">
        <obo:RO_0001025 rdf:resource="http://purl.obolibrary.org/obo/GAZ_00000540"/>
        <obo:IAO_0000115>A stratovolcano or large lava-dome complex of mostly Pleistocene age. It is located about 50 km ESE of Guatemala City, about 20 km south of the main volcanic chain. An ancestral andesitic stratovolcano, Miraflores, was formed about 100,000 years ago. Tecuamburro and other lava domes were constructed during the late Pleistocene or early Holocene within a horseshoe-shaped, east-facing caldera produced by structural failure of the older Miraflores stratovolcano prior to about 38,000 years ago. One of the largest of these domes, Pena Blanca, overtops the NW rim of the collapse scarp. Two nested craters, the larger of which is Chupadero, lie at the NW end of the complex. The smaller crater is a phreatic tuff ring, Laguna Ixpaco, that was formed about 2900 years ago during the latest dated eruption of the Tecuamburro complex. Numerous fumaroles, hot springs, and boiling mud pots are found in the area around the acidic lake.</obo:IAO_0000115>
        <oboInOwl:hasOBONamespace>GAZ</oboInOwl:hasOBONamespace>
        <oboInOwl:id>GAZ:00056117</oboInOwl:id>
        <rdfs:label>Vulcan Tecuamburro</rdfs:label>
    </owl:NamedIndividual>
    


    <!-- http://purl.obolibrary.org/obo/GAZ_00056118 -->

    <owl:NamedIndividual rdf:about="http://purl.obolibrary.org/obo/GAZ_00056118">
        <obo:RO_0001025 rdf:resource="http://purl.obolibrary.org/obo/GAZ_00000540"/>
        <obo:IAO_0000115>A small basaltic stratovolcano located NNE of the city of Cuilapa, north of the major NW-SE-trending Jalpatagua fault that cuts diagonally across SE Guatemala. The 1815 m high volcano was constructed near the SE rim of the large Miocene Santa Rosa de Lima caldera. Jumaytepeque volcano is not overlain by a ca. 23,000-year-old tephra unit from nearby Ayarza caldera, and its erosionally unmodified form suggests that Holocene activity is possible. Two older cinder cones to the north are covered with Ayarza tephra.</obo:IAO_0000115>
        <oboInOwl:hasOBONamespace>GAZ</oboInOwl:hasOBONamespace>
        <oboInOwl:id>GAZ:00056118</oboInOwl:id>
        <rdfs:label>Jumaytepeque Volcano</rdfs:label>
    </owl:NamedIndividual>
    


    <!-- http://purl.obolibrary.org/obo/GAZ_00056119 -->

    <owl:NamedIndividual rdf:about="http://purl.obolibrary.org/obo/GAZ_00056119">
        <obo:RO_0001025 rdf:resource="http://purl.obolibrary.org/obo/GAZ_00000499"/>
        <obo:IAO_0000115>The easternmost of a chain of large stratovolcanoes extending along the volcanic front of Guatemala. Like Tecuamburro volcano, Moyuta is offset about 20 km south of the main volcanic chain and lies south of the Jalpatagua Fault, overlying the southern boundary of the Jalpatagua Graben. The 1662 m high volcano is capped by a cluster of at least three forested, steep-sided, coalescing andesitic lava domes that from some distant perspectives give the summit a flat-topped appearance. Numerous cinder cones in various stages of erosion are located on the flanks of the complex. The age of the latest eruption of Moyuta volcano is not known, although the summit domes were considered to have been emplaced in relatively recent times (Williams et al., 1964). Small fumaroles are found on the northern and southern flanks of the volcano, and hot springs are located near Azulco at the NE base and along rivers on the SE side of Moyuta.</obo:IAO_0000115>
        <oboInOwl:hasOBONamespace>GAZ</oboInOwl:hasOBONamespace>
        <oboInOwl:id>GAZ:00056119</oboInOwl:id>
        <rdfs:label>Moyuta Volcano</rdfs:label>
    </owl:NamedIndividual>
    


    <!-- http://purl.obolibrary.org/obo/GAZ_00056120 -->

    <owl:NamedIndividual rdf:about="http://purl.obolibrary.org/obo/GAZ_00056120">
        <obo:RO_0001025 rdf:resource="http://purl.obolibrary.org/obo/GAZ_00000499"/>
        <obo:IAO_0000115>A stratovolcano in southeastern Guatemala, on the border with El Salvador.</obo:IAO_0000115>
        <oboInOwl:hasOBONamespace>GAZ</oboInOwl:hasOBONamespace>
        <oboInOwl:id>GAZ:00056120</oboInOwl:id>
        <rdfs:label>Chingo Volcano</rdfs:label>
    </owl:NamedIndividual>
    


    <!-- http://purl.obolibrary.org/obo/GAZ_00056125 -->

    <owl:NamedIndividual rdf:about="http://purl.obolibrary.org/obo/GAZ_00056125">
        <obo:RO_0001025 rdf:resource="http://purl.obolibrary.org/obo/GAZ_00000499"/>
        <obo:IAO_0000115>A stratovolcano that rises about 700 m above plains south of the town of Monjas. The summit of the 1716 m high forested stratovolcano is cut by a broad erosional crater that extends to the base of the volcano and is narrowly breached to the NE. A Holocene pyroclastic cone near the NE base of Volcan Tahual fed a short basaltic lava flow (Williams et al., 1964). The scenic lake-filled Laguna de Hoyo lies north of the volcano. This steep-walled crater and the NE-flank cinder cone lie along faults bordering a graben that extends across the eastern base of the volcano to neighboring Retana caldera on the SE.</obo:IAO_0000115>
        <oboInOwl:hasOBONamespace>GAZ</oboInOwl:hasOBONamespace>
        <oboInOwl:id>GAZ:00056125</oboInOwl:id>
        <rdfs:label>Tahual Volcano</rdfs:label>
    </owl:NamedIndividual>
    


    <!-- http://purl.obolibrary.org/obo/GAZ_00056126 -->

    <owl:NamedIndividual rdf:about="http://purl.obolibrary.org/obo/GAZ_00056126">
        <obo:RO_0001025 rdf:resource="http://purl.obolibrary.org/obo/GAZ_00000439"/>
        <obo:IAO_0000115>A series of youthful lava flows was erupted from vents cutting through Tertiary pyroclastic rocks WNW of Ipala volcano about 5 km south of the town of Quezaltepeque. These basaltic flows issued passively from vents along a N-S-trending fault without accompanying explosive activity. The vents are capped by low mounds of lava. The flows were considered to be of Holocene age by Williams et al. (1964).</obo:IAO_0000115>
        <oboInOwl:hasOBONamespace>GAZ</oboInOwl:hasOBONamespace>
        <oboInOwl:id>GAZ:00056126</oboInOwl:id>
        <rdfs:label>Quezaltepeque Volcanic Field</rdfs:label>
    </owl:NamedIndividual>
    


    <!-- http://purl.obolibrary.org/obo/GAZ_00056127 -->

    <owl:NamedIndividual rdf:about="http://purl.obolibrary.org/obo/GAZ_00056127">
        <obo:RO_0001025 rdf:resource="http://purl.obolibrary.org/obo/GAZ_00000541"/>
        <obo:IAO_0000115>A stratovolcano in Guatemala, on the shores of Lago de Atitlan. At its base is a village of the same name.</obo:IAO_0000115>
        <oboInOwl:hasOBONamespace>GAZ</oboInOwl:hasOBONamespace>
        <oboInOwl:id>GAZ:00056127</oboInOwl:id>
        <rdfs:label>Volcan San Pedro</rdfs:label>
    </owl:NamedIndividual>
    


    <!-- http://purl.obolibrary.org/obo/GAZ_00056128 -->

    <owl:NamedIndividual rdf:about="http://purl.obolibrary.org/obo/GAZ_00056128">
        <obo:RO_0001025 rdf:resource="http://purl.obolibrary.org/obo/GAZ_00000499"/>
        <obo:IAO_0000115>One of the largest of a cluster of small stratovolcanoes located in SE Guatemala behind the volcanic front. Volcan de Flores, also known as Volcan Amayo, lies about 10 km west of the city of Jutiapa, at the SW end of the SE Guatemala volcanic platform. The 1600 m high summit rises up to 600 m above a basement of Cretaceous and Tertiary sedimentary rocks and contains a shallow crater breached on its eastern side. Satellitic cones occur at the southern and eastern base of the dominantly basaltic Flores volcano. Youthful lava flows occur at the NE base of the volcano, near El Aguacite.</obo:IAO_0000115>
        <oboInOwl:hasOBONamespace>GAZ</oboInOwl:hasOBONamespace>
        <oboInOwl:id>GAZ:00056128</oboInOwl:id>
        <rdfs:label>Volcan de Flores</rdfs:label>
    </owl:NamedIndividual>
    


    <!-- http://purl.obolibrary.org/obo/GAZ_00056129 -->

    <owl:NamedIndividual rdf:about="http://purl.obolibrary.org/obo/GAZ_00056129">
        <obo:RO_0001025 rdf:resource="http://purl.obolibrary.org/obo/GAZ_00000499"/>
        <obo:IAO_0000115>A cluster of cinder cones and low shield volcanoes surrounds the city of Jutiapa in SE Guatemala. The most prominent feature is Cerro Santiago, one of two coalescing cinder cones capping a low shield volcano SE of Jutiapa. Youthful flows from the twin Los Cerritos cones NE of Jutiapa cross the Interamerican highway. Volcan Culma forms a steep-sided basaltic lava mound immediately east of the city. To the west lies Cerro Gordo (referred to by Williams et al., 1964 as Volcano Amayo), a craterless cinder cone surrounded by basaltic lava flows. It is one of several cinder cones to have produced lava flows that blanket the landscape between Jutiapa and Tertiary volcanic hills to the south.</obo:IAO_0000115>
        <oboInOwl:hasOBONamespace>GAZ</oboInOwl:hasOBONamespace>
        <oboInOwl:id>GAZ:00056129</oboInOwl:id>
        <rdfs:label>Cerro Santiago</rdfs:label>
    </owl:NamedIndividual>
    


    <!-- http://purl.obolibrary.org/obo/GAZ_00056130 -->

    <owl:NamedIndividual rdf:about="http://purl.obolibrary.org/obo/GAZ_00056130">
        <obo:RO_0001025 rdf:resource="http://purl.obolibrary.org/obo/GAZ_00000499"/>
        <obo:IAO_0000115>One of the largest volcanoes in SE Guatemala. The 2042 m high summit of the andesitic-to-basaltic stratovolcano is elongated in a N-S direction. Several large canyons cut the slopes of the dominantly andesitic edifice. A large parasitic cone, Cerro Mataltepe, is located on the upper northern flank, and two smaller cones are located on the lower northern flank. Two basaltic lava flows of Holocene age are located on the northern and NW flanks (Williams et al., 1964), and many flank vents are basaltic. Suchitan was constructed immediately to the east of the 5 km wide basaltic-to-dacitic Retana caldera, formed in part in association with the eruption of a dacitic pumice deposit. Steep walls 60-250-m high rise above the flat caldera floor. One of the latest basaltic lava flows from Suchitan flowed through a low notch in the eastern caldera rim. Several lava cones and a maar are located along a N-S line north of Retana caldera. A reported eruption of Suchitan in 1469 is considered to have actually been from Atitlan volcano in the Guatemalan highlands.</obo:IAO_0000115>
        <oboInOwl:hasOBONamespace>GAZ</oboInOwl:hasOBONamespace>
        <oboInOwl:id>GAZ:00056130</oboInOwl:id>
        <rdfs:label>Volcan Suchitan</rdfs:label>
    </owl:NamedIndividual>
    


    <!-- http://purl.obolibrary.org/obo/GAZ_00056132 -->

    <owl:NamedIndividual rdf:about="http://purl.obolibrary.org/obo/GAZ_00056132">
        <obo:RO_0001025 rdf:resource="http://purl.obolibrary.org/obo/GAZ_00000499"/>
        <obo:IAO_0000115>A 4 x 5 km wide rhyolitic obsidian lava field was erupted within the Ipala graben from a craterless vent along a NE-trending fissure that passes through adjacent rhyolitic lava domes and basaltic cinder cones. Obsidian from Ixtepeque has shown up at archaeological sites across Central America. Flat-lying pumice beds produced by explosive eruptions preceding lava effusion are found locally around the volcano. Other obsidian flows originated from lava domes NE of Ixtepeque. These rhyolitic vents are interspersed with basaltic cinder cones and lava flows. Laguna de Obrajuelo is a complex cone cut by a large crater more than a km in diameter.</obo:IAO_0000115>
        <oboInOwl:hasOBONamespace>GAZ</oboInOwl:hasOBONamespace>
        <oboInOwl:id>GAZ:00056132</oboInOwl:id>
        <rdfs:label>Ixtepeque Volcano</rdfs:label>
    </owl:NamedIndividual>
    


    <!-- http://purl.obolibrary.org/obo/GAZ_00056133 -->

    <owl:NamedIndividual rdf:about="http://purl.obolibrary.org/obo/GAZ_00056133">
        <obo:RO_0001025 rdf:resource="http://purl.obolibrary.org/obo/GAZ_00000446"/>
        <obo:IAO_0000115>A stratovolcano that extends nearly across the full width of the Ipala graben and rises 750 m above the graben floor. The 1650 m high summit of Volcan Ipala is truncated by a 1 km wide crater whose steep, 150 m high walls tower above a lake. A prominent parasitic cone, Monte Rico, is located on the southern flank; it and other cones on the northern flank lie along a N-S-trending fracture that continues well beyond the southern flank of the volcano. The eastern flank of Ipala is cut by a 17 km long, NNE-SSW fissure that produced a conspicuous line of Holocene cinder cones that fed basaltic lava flows covering about 20 sq km.</obo:IAO_0000115>
        <oboInOwl:hasOBONamespace>GAZ</oboInOwl:hasOBONamespace>
        <oboInOwl:id>GAZ:00056133</oboInOwl:id>
        <rdfs:label>Volcan Ipala</rdfs:label>
    </owl:NamedIndividual>
    


    <!-- http://purl.obolibrary.org/obo/GAZ_00056134 -->

    <owl:NamedIndividual rdf:about="http://purl.obolibrary.org/obo/GAZ_00056134">
        <obo:RO_0001025 rdf:resource="http://purl.obolibrary.org/obo/GAZ_00000446"/>
        <obo:IAO_0000115>A volcanic field that occupies a fault-bounded basin underlain by Cretaceous plutonic rocks in the Chiquimula Valley of SE Guatemala. Initial eruptions during the Pleistocene produced mesa-forming basaltic lava flows along the N-S-trending fault forming the eastern edge of the Ipala graben. These were followed by the eruption of widespread lava flows NW of Chiquimula town that covered about 12 sq km. The most recent eruptions produced basaltic cinder cones and lava flows near the northern edge of Chiquimula town. The cinder cones were constructed along a N-S-trending fracture, with Cerro Grande at the northern end being the largest and Cerro Chiquito at the southern end being the youngest. The lava flows from Cerro Chiquito are so fresh and sparsely vegetated they were considered by Williams et al. (1964) to possibly be less than 1000 years old.</obo:IAO_0000115>
        <oboInOwl:hasOBONamespace>GAZ</oboInOwl:hasOBONamespace>
        <oboInOwl:id>GAZ:00056134</oboInOwl:id>
        <rdfs:label>Chiquimula Volcanic Field</rdfs:label>
    </owl:NamedIndividual>
    


    <!-- http://purl.obolibrary.org/obo/GAZ_00056628 -->

    <owl:NamedIndividual rdf:about="http://purl.obolibrary.org/obo/GAZ_00056628">
        <obo:IAO_0000115>A nature reserve in south-central Belize. The Cockscomb Basin Wildlife Sanctuary is actually comprised by two adjacent geographic basins. The West Basin is drained by the Swasey Branch, which is one of the main tributaries to the Monkey River. The East Basin consists of the upper watershed of South Stann Creek. The West Basin, being more difficult to access given distance from trailheads and higher forest density, is as of the current time still relatively unexplored from the standpoint of species mapping.</obo:IAO_0000115>
        <oboInOwl:hasOBONamespace>GAZ</oboInOwl:hasOBONamespace>
        <oboInOwl:id>GAZ:00056628</oboInOwl:id>
        <rdfs:label>Cockscomb Basin Wildlife Sanctuary</rdfs:label>
    </owl:NamedIndividual>
    


    <!-- http://purl.obolibrary.org/obo/GAZ_00062332 -->

    <owl:NamedIndividual rdf:about="http://purl.obolibrary.org/obo/GAZ_00062332">
        <obo:RO_0001025 rdf:resource="http://purl.obolibrary.org/obo/GAZ_00000494"/>
        <obo:IAO_0000115>A lake in Guatemala. The Polochic river is the largest river that drains into the lake. The lake drains into the Caribbean Sea through the smaller Golfete Dulce and the Rio Dulce.</obo:IAO_0000115>
        <oboInOwl:hasOBONamespace>GAZ</oboInOwl:hasOBONamespace>
        <oboInOwl:id>GAZ:00062332</oboInOwl:id>
        <rdfs:label>Lago de Izabal</rdfs:label>
    </owl:NamedIndividual>
    


    <!-- http://purl.obolibrary.org/obo/GAZ_00062333 -->

    <owl:NamedIndividual rdf:about="http://purl.obolibrary.org/obo/GAZ_00062333">
        <obo:RO_0001025 rdf:resource="http://purl.obolibrary.org/obo/GAZ_00062334"/>
        <obo:IAO_0000115>A crater lake located near the town of San Martin Sacatepequez in the department of Quetzaltenango.</obo:IAO_0000115>
        <oboInOwl:hasOBONamespace>GAZ</oboInOwl:hasOBONamespace>
        <oboInOwl:id>GAZ:00062333</oboInOwl:id>
        <rdfs:label>Laguna Chicabal</rdfs:label>
    </owl:NamedIndividual>
    


    <!-- http://purl.obolibrary.org/obo/GAZ_00062334 -->

    <owl:NamedIndividual rdf:about="http://purl.obolibrary.org/obo/GAZ_00062334">
        <obo:RO_0001025 rdf:resource="http://purl.obolibrary.org/obo/GAZ_00068184"/>
        <oboInOwl:hasOBONamespace>GAZ</oboInOwl:hasOBONamespace>
        <oboInOwl:id>GAZ:00062334</oboInOwl:id>
        <rdfs:label>Volcan Chicabal</rdfs:label>
    </owl:NamedIndividual>
    


    <!-- http://purl.obolibrary.org/obo/GAZ_00062335 -->

    <owl:NamedIndividual rdf:about="http://purl.obolibrary.org/obo/GAZ_00062335">
        <obo:RO_0001025 rdf:resource="http://purl.obolibrary.org/obo/GAZ_00000508"/>
        <obo:RO_0001025 rdf:resource="http://purl.obolibrary.org/obo/GAZ_00266062"/>
        <obo:IAO_0000115>A freshwater lake in central Peten department in Guatemala.</obo:IAO_0000115>
        <oboInOwl:hasOBONamespace>GAZ</oboInOwl:hasOBONamespace>
        <oboInOwl:id>GAZ:00062335</oboInOwl:id>
        <rdfs:label>Lago Peten Itza</rdfs:label>
    </owl:NamedIndividual>
    


    <!-- http://purl.obolibrary.org/obo/GAZ_00062336 -->

    <owl:NamedIndividual rdf:about="http://purl.obolibrary.org/obo/GAZ_00062336">
        <obo:RO_0001025 rdf:resource="http://purl.obolibrary.org/obo/GAZ_00062335"/>
        <obo:IAO_0000115>An island in Lago Peten Itza, now connected to the shore by a causeway.</obo:IAO_0000115>
        <oboInOwl:hasOBONamespace>GAZ</oboInOwl:hasOBONamespace>
        <oboInOwl:id>GAZ:00062336</oboInOwl:id>
        <rdfs:label>Island of Flores</rdfs:label>
    </owl:NamedIndividual>
    


    <!-- http://purl.obolibrary.org/obo/GAZ_00062337 -->

    <owl:NamedIndividual rdf:about="http://purl.obolibrary.org/obo/GAZ_00062337">
        <rdf:type rdf:resource="http://purl.obolibrary.org/obo/ENVO_00000856"/>
        <obo:RO_0001025 rdf:resource="http://purl.obolibrary.org/obo/GAZ_00062336"/>
        <obo:IAO_0000115>A municipality in the Department of Peten. Located on the Island of Flores in Lago Peten Itza.</obo:IAO_0000115>
        <oboInOwl:hasOBONamespace>GAZ</oboInOwl:hasOBONamespace>
        <oboInOwl:id>GAZ:00062337</oboInOwl:id>
        <rdfs:label>Municipality of Flores</rdfs:label>
    </owl:NamedIndividual>
    


    <!-- http://purl.obolibrary.org/obo/GAZ_00067906 -->

    <owl:NamedIndividual rdf:about="http://purl.obolibrary.org/obo/GAZ_00067906">
        <rdf:type rdf:resource="http://purl.obolibrary.org/obo/ENVO_00000856"/>
        <obo:RO_0001025 rdf:resource="http://purl.obolibrary.org/obo/GAZ_00000430"/>
        <obo:IAO_0000115>A municipality in the Guatemalan Department of Alta Verapaz.</obo:IAO_0000115>
        <oboInOwl:hasOBONamespace>GAZ</oboInOwl:hasOBONamespace>
        <oboInOwl:id>GAZ:00067906</oboInOwl:id>
        <rdfs:label>Municipality of Chisec</rdfs:label>
    </owl:NamedIndividual>
    


    <!-- http://purl.obolibrary.org/obo/GAZ_00068050 -->

    <owl:NamedIndividual rdf:about="http://purl.obolibrary.org/obo/GAZ_00068050">
        <obo:IAO_0000115>A lake formed by the Cerron Grande dam on the Rio Lempa.</obo:IAO_0000115>
        <oboInOwl:hasOBONamespace>GAZ</oboInOwl:hasOBONamespace>
        <oboInOwl:id>GAZ:00068050</oboInOwl:id>
        <rdfs:label>Lago de Suchitlan</rdfs:label>
    </owl:NamedIndividual>
    


    <!-- http://purl.obolibrary.org/obo/GAZ_00068052 -->

    <owl:NamedIndividual rdf:about="http://purl.obolibrary.org/obo/GAZ_00068052">
        <rdf:type rdf:resource="http://purl.obolibrary.org/obo/ENVO_00000856"/>
        <obo:RO_0001025 rdf:resource="http://purl.obolibrary.org/obo/GAZ_00000430"/>
        <obo:IAO_0000115>A municipality in the Guatemalan Department of Alta Verapaz.</obo:IAO_0000115>
        <oboInOwl:hasOBONamespace>GAZ</oboInOwl:hasOBONamespace>
        <oboInOwl:id>GAZ:00068052</oboInOwl:id>
        <rdfs:label>Municipality of Santa Maria Cahabon</rdfs:label>
    </owl:NamedIndividual>
    


    <!-- http://purl.obolibrary.org/obo/GAZ_00068053 -->

    <owl:NamedIndividual rdf:about="http://purl.obolibrary.org/obo/GAZ_00068053">
        <rdf:type rdf:resource="http://purl.obolibrary.org/obo/ENVO_00000856"/>
        <obo:RO_0001025 rdf:resource="http://purl.obolibrary.org/obo/GAZ_00000430"/>
        <obo:IAO_0000115>A municipality in the Guatemalan Department of Alta Verapaz.</obo:IAO_0000115>
        <oboInOwl:hasOBONamespace>GAZ</oboInOwl:hasOBONamespace>
        <oboInOwl:id>GAZ:00068053</oboInOwl:id>
        <rdfs:label>Municipality of Coban</rdfs:label>
    </owl:NamedIndividual>
    


    <!-- http://purl.obolibrary.org/obo/GAZ_00068054 -->

    <owl:NamedIndividual rdf:about="http://purl.obolibrary.org/obo/GAZ_00068054">
        <rdf:type rdf:resource="http://purl.obolibrary.org/obo/ENVO_00000856"/>
        <obo:RO_0001025 rdf:resource="http://purl.obolibrary.org/obo/GAZ_00000430"/>
        <obo:IAO_0000115>A municipality in the Guatemalan Department of Alta Verapaz.</obo:IAO_0000115>
        <oboInOwl:hasOBONamespace>GAZ</oboInOwl:hasOBONamespace>
        <oboInOwl:id>GAZ:00068054</oboInOwl:id>
        <rdfs:label>Municipality of Santa Cruz Verapaz</rdfs:label>
    </owl:NamedIndividual>
    


    <!-- http://purl.obolibrary.org/obo/GAZ_00068055 -->

    <owl:NamedIndividual rdf:about="http://purl.obolibrary.org/obo/GAZ_00068055">
        <rdf:type rdf:resource="http://purl.obolibrary.org/obo/ENVO_00000856"/>
        <obo:RO_0001025 rdf:resource="http://purl.obolibrary.org/obo/GAZ_00000430"/>
        <obo:IAO_0000115>A municipality in the Guatemalan Department of Alta Verapaz.</obo:IAO_0000115>
        <oboInOwl:hasOBONamespace>GAZ</oboInOwl:hasOBONamespace>
        <oboInOwl:id>GAZ:00068055</oboInOwl:id>
        <rdfs:label>Municipality of Fray Bartolome de las Casas</rdfs:label>
    </owl:NamedIndividual>
    


    <!-- http://purl.obolibrary.org/obo/GAZ_00068056 -->

    <owl:NamedIndividual rdf:about="http://purl.obolibrary.org/obo/GAZ_00068056">
        <rdf:type rdf:resource="http://purl.obolibrary.org/obo/ENVO_00000856"/>
        <obo:RO_0001025 rdf:resource="http://purl.obolibrary.org/obo/GAZ_00000430"/>
        <obo:IAO_0000115>A municipality in the Guatemalan Department of Alta Verapaz.</obo:IAO_0000115>
        <oboInOwl:hasOBONamespace>GAZ</oboInOwl:hasOBONamespace>
        <oboInOwl:id>GAZ:00068056</oboInOwl:id>
        <rdfs:label>Municipality of Senahu</rdfs:label>
    </owl:NamedIndividual>
    


    <!-- http://purl.obolibrary.org/obo/GAZ_00068057 -->

    <owl:NamedIndividual rdf:about="http://purl.obolibrary.org/obo/GAZ_00068057">
        <rdf:type rdf:resource="http://purl.obolibrary.org/obo/ENVO_00000856"/>
        <obo:RO_0001025 rdf:resource="http://purl.obolibrary.org/obo/GAZ_00000430"/>
        <obo:IAO_0000115>A municipality in the Guatemalan Department of Alta Verapaz.</obo:IAO_0000115>
        <oboInOwl:hasOBONamespace>GAZ</oboInOwl:hasOBONamespace>
        <oboInOwl:id>GAZ:00068057</oboInOwl:id>
        <rdfs:label>Municipality of Santa Catalina La Tinta</rdfs:label>
    </owl:NamedIndividual>
    


    <!-- http://purl.obolibrary.org/obo/GAZ_00068058 -->

    <owl:NamedIndividual rdf:about="http://purl.obolibrary.org/obo/GAZ_00068058">
        <rdf:type rdf:resource="http://purl.obolibrary.org/obo/ENVO_00000856"/>
        <obo:RO_0001025 rdf:resource="http://purl.obolibrary.org/obo/GAZ_00000430"/>
        <obo:IAO_0000115>A municipality in the Guatemalan Department of Alta Verapaz.</obo:IAO_0000115>
        <oboInOwl:hasOBONamespace>GAZ</oboInOwl:hasOBONamespace>
        <oboInOwl:id>GAZ:00068058</oboInOwl:id>
        <rdfs:label>Municipality of Chahal</rdfs:label>
    </owl:NamedIndividual>
    


    <!-- http://purl.obolibrary.org/obo/GAZ_00068059 -->

    <owl:NamedIndividual rdf:about="http://purl.obolibrary.org/obo/GAZ_00068059">
        <rdf:type rdf:resource="http://purl.obolibrary.org/obo/ENVO_00000856"/>
        <obo:RO_0001025 rdf:resource="http://purl.obolibrary.org/obo/GAZ_00000430"/>
        <obo:IAO_0000115>A municipality in the Guatemalan Department of Alta Verapaz.</obo:IAO_0000115>
        <oboInOwl:hasOBONamespace>GAZ</oboInOwl:hasOBONamespace>
        <oboInOwl:id>GAZ:00068059</oboInOwl:id>
        <rdfs:label>Municipality of Lanquin</rdfs:label>
    </owl:NamedIndividual>
    


    <!-- http://purl.obolibrary.org/obo/GAZ_00068060 -->

    <owl:NamedIndividual rdf:about="http://purl.obolibrary.org/obo/GAZ_00068060">
        <rdf:type rdf:resource="http://purl.obolibrary.org/obo/ENVO_00000856"/>
        <obo:RO_0001025 rdf:resource="http://purl.obolibrary.org/obo/GAZ_00000430"/>
        <obo:IAO_0000115>A municipality in the Guatemalan D/epartment of Alta Verapaz.</obo:IAO_0000115>
        <oboInOwl:hasOBONamespace>GAZ</oboInOwl:hasOBONamespace>
        <oboInOwl:id>GAZ:00068060</oboInOwl:id>
        <rdfs:label>Municipality of San Juan Chamelco</rdfs:label>
    </owl:NamedIndividual>
    


    <!-- http://purl.obolibrary.org/obo/GAZ_00068061 -->

    <owl:NamedIndividual rdf:about="http://purl.obolibrary.org/obo/GAZ_00068061">
        <rdf:type rdf:resource="http://purl.obolibrary.org/obo/ENVO_00000856"/>
        <obo:RO_0001025 rdf:resource="http://purl.obolibrary.org/obo/GAZ_00000430"/>
        <obo:IAO_0000115>A municipality in the Guatemalan Department of Alta Verapaz.</obo:IAO_0000115>
        <oboInOwl:hasOBONamespace>GAZ</oboInOwl:hasOBONamespace>
        <oboInOwl:id>GAZ:00068061</oboInOwl:id>
        <rdfs:label>Municipality of Tactic</rdfs:label>
    </owl:NamedIndividual>
    


    <!-- http://purl.obolibrary.org/obo/GAZ_00068062 -->

    <owl:NamedIndividual rdf:about="http://purl.obolibrary.org/obo/GAZ_00068062">
        <rdf:type rdf:resource="http://purl.obolibrary.org/obo/ENVO_00000856"/>
        <obo:RO_0001025 rdf:resource="http://purl.obolibrary.org/obo/GAZ_00000430"/>
        <obo:IAO_0000115>A municipality in the Guatemalan Department of Alta Verapaz.</obo:IAO_0000115>
        <oboInOwl:hasOBONamespace>GAZ</oboInOwl:hasOBONamespace>
        <oboInOwl:id>GAZ:00068062</oboInOwl:id>
        <rdfs:label>Municipality of Tamahu</rdfs:label>
    </owl:NamedIndividual>
    


    <!-- http://purl.obolibrary.org/obo/GAZ_00068063 -->

    <owl:NamedIndividual rdf:about="http://purl.obolibrary.org/obo/GAZ_00068063">
        <rdf:type rdf:resource="http://purl.obolibrary.org/obo/ENVO_00000856"/>
        <obo:RO_0001025 rdf:resource="http://purl.obolibrary.org/obo/GAZ_00000430"/>
        <obo:IAO_0000115>A municipality in the Guatemalan Department of Alta Verapaz.</obo:IAO_0000115>
        <oboInOwl:hasOBONamespace>GAZ</oboInOwl:hasOBONamespace>
        <oboInOwl:id>GAZ:00068063</oboInOwl:id>
        <rdfs:label>Municipality of San Cristobal Verapaz</rdfs:label>
    </owl:NamedIndividual>
    


    <!-- http://purl.obolibrary.org/obo/GAZ_00068064 -->

    <owl:NamedIndividual rdf:about="http://purl.obolibrary.org/obo/GAZ_00068064">
        <rdf:type rdf:resource="http://purl.obolibrary.org/obo/ENVO_00000856"/>
        <obo:RO_0001025 rdf:resource="http://purl.obolibrary.org/obo/GAZ_00000430"/>
        <obo:IAO_0000115>A municipality in the Guatemalan Department of Alta Verapaz.</obo:IAO_0000115>
        <oboInOwl:hasOBONamespace>GAZ</oboInOwl:hasOBONamespace>
        <oboInOwl:id>GAZ:00068064</oboInOwl:id>
        <rdfs:label>Municipality of Tucuru</rdfs:label>
    </owl:NamedIndividual>
    


    <!-- http://purl.obolibrary.org/obo/GAZ_00068065 -->

    <owl:NamedIndividual rdf:about="http://purl.obolibrary.org/obo/GAZ_00068065">
        <rdf:type rdf:resource="http://purl.obolibrary.org/obo/ENVO_00000856"/>
        <obo:RO_0001025 rdf:resource="http://purl.obolibrary.org/obo/GAZ_00000433"/>
        <obo:IAO_0000115>A municipality in the Baja Verapaz Department of Guatemala.</obo:IAO_0000115>
        <oboInOwl:hasOBONamespace>GAZ</oboInOwl:hasOBONamespace>
        <oboInOwl:id>GAZ:00068065</oboInOwl:id>
        <rdfs:label>Municipality of San Miguel Chicaj</rdfs:label>
    </owl:NamedIndividual>
    


    <!-- http://purl.obolibrary.org/obo/GAZ_00068066 -->

    <owl:NamedIndividual rdf:about="http://purl.obolibrary.org/obo/GAZ_00068066">
        <rdf:type rdf:resource="http://purl.obolibrary.org/obo/ENVO_00000856"/>
        <obo:RO_0001025 rdf:resource="http://purl.obolibrary.org/obo/GAZ_00000433"/>
        <obo:IAO_0000115>A municipality in the Baja Verapaz Department of Guatemala.</obo:IAO_0000115>
        <oboInOwl:hasOBONamespace>GAZ</oboInOwl:hasOBONamespace>
        <oboInOwl:id>GAZ:00068066</oboInOwl:id>
        <rdfs:label>Municipality of Granados</rdfs:label>
    </owl:NamedIndividual>
    


    <!-- http://purl.obolibrary.org/obo/GAZ_00068067 -->

    <owl:NamedIndividual rdf:about="http://purl.obolibrary.org/obo/GAZ_00068067">
        <rdf:type rdf:resource="http://purl.obolibrary.org/obo/ENVO_00000856"/>
        <obo:RO_0001025 rdf:resource="http://purl.obolibrary.org/obo/GAZ_00000433"/>
        <obo:IAO_0000115>A municipality in the Baja Verapaz Department of Guatemala.</obo:IAO_0000115>
        <oboInOwl:hasOBONamespace>GAZ</oboInOwl:hasOBONamespace>
        <oboInOwl:id>GAZ:00068067</oboInOwl:id>
        <rdfs:label>Municipality of Rabinal</rdfs:label>
    </owl:NamedIndividual>
    


    <!-- http://purl.obolibrary.org/obo/GAZ_00068068 -->

    <owl:NamedIndividual rdf:about="http://purl.obolibrary.org/obo/GAZ_00068068">
        <rdf:type rdf:resource="http://purl.obolibrary.org/obo/ENVO_00000856"/>
        <obo:RO_0001025 rdf:resource="http://purl.obolibrary.org/obo/GAZ_00000433"/>
        <obo:IAO_0000115>A municipality in the Baja Verapaz Department of Guatemala.</obo:IAO_0000115>
        <oboInOwl:hasOBONamespace>GAZ</oboInOwl:hasOBONamespace>
        <oboInOwl:id>GAZ:00068068</oboInOwl:id>
        <rdfs:label>Municipality of Cubulco</rdfs:label>
    </owl:NamedIndividual>
    


    <!-- http://purl.obolibrary.org/obo/GAZ_00068069 -->

    <owl:NamedIndividual rdf:about="http://purl.obolibrary.org/obo/GAZ_00068069">
        <rdf:type rdf:resource="http://purl.obolibrary.org/obo/ENVO_00000856"/>
        <obo:RO_0001025 rdf:resource="http://purl.obolibrary.org/obo/GAZ_00000433"/>
        <obo:IAO_0000115>A municipality in the Baja Verapaz Department of Guatemala.</obo:IAO_0000115>
        <oboInOwl:hasOBONamespace>GAZ</oboInOwl:hasOBONamespace>
        <oboInOwl:id>GAZ:00068069</oboInOwl:id>
        <rdfs:label>Municipality of San Jeronimo</rdfs:label>
    </owl:NamedIndividual>
    


    <!-- http://purl.obolibrary.org/obo/GAZ_00068070 -->

    <owl:NamedIndividual rdf:about="http://purl.obolibrary.org/obo/GAZ_00068070">
        <rdf:type rdf:resource="http://purl.obolibrary.org/obo/ENVO_00000856"/>
        <obo:RO_0001025 rdf:resource="http://purl.obolibrary.org/obo/GAZ_00000433"/>
        <obo:IAO_0000115>A municipality in the Baja Verapaz Department of Guatemala.</obo:IAO_0000115>
        <oboInOwl:hasOBONamespace>GAZ</oboInOwl:hasOBONamespace>
        <oboInOwl:id>GAZ:00068070</oboInOwl:id>
        <rdfs:label>Municipality of Santa Cruz El Chol</rdfs:label>
    </owl:NamedIndividual>
    


    <!-- http://purl.obolibrary.org/obo/GAZ_00068071 -->

    <owl:NamedIndividual rdf:about="http://purl.obolibrary.org/obo/GAZ_00068071">
        <rdf:type rdf:resource="http://purl.obolibrary.org/obo/ENVO_00000856"/>
        <obo:RO_0001025 rdf:resource="http://purl.obolibrary.org/obo/GAZ_00000439"/>
        <obo:IAO_0000115>A municipality in the Chimaltenango Department of Guatemala.</obo:IAO_0000115>
        <oboInOwl:hasOBONamespace>GAZ</oboInOwl:hasOBONamespace>
        <oboInOwl:id>GAZ:00068071</oboInOwl:id>
        <rdfs:label>Municipality of Tecpan Guatemala</rdfs:label>
    </owl:NamedIndividual>
    


    <!-- http://purl.obolibrary.org/obo/GAZ_00068072 -->

    <owl:NamedIndividual rdf:about="http://purl.obolibrary.org/obo/GAZ_00068072">
        <rdf:type rdf:resource="http://purl.obolibrary.org/obo/ENVO_00000856"/>
        <obo:RO_0001025 rdf:resource="http://purl.obolibrary.org/obo/GAZ_00000439"/>
        <obo:IAO_0000115>A municipality in the Chimaltenango Department of Guatemala.</obo:IAO_0000115>
        <oboInOwl:hasOBONamespace>GAZ</oboInOwl:hasOBONamespace>
        <oboInOwl:id>GAZ:00068072</oboInOwl:id>
        <rdfs:label>Municipality of Parramos</rdfs:label>
    </owl:NamedIndividual>
    


    <!-- http://purl.obolibrary.org/obo/GAZ_00068073 -->

    <owl:NamedIndividual rdf:about="http://purl.obolibrary.org/obo/GAZ_00068073">
        <rdf:type rdf:resource="http://purl.obolibrary.org/obo/ENVO_00000856"/>
        <obo:RO_0001025 rdf:resource="http://purl.obolibrary.org/obo/GAZ_00000439"/>
        <obo:IAO_0000115>A municipality in the Chimaltenango Department of Guatemala.</obo:IAO_0000115>
        <oboInOwl:hasOBONamespace>GAZ</oboInOwl:hasOBONamespace>
        <oboInOwl:id>GAZ:00068073</oboInOwl:id>
        <rdfs:label>Municipality of Zaragoza</rdfs:label>
    </owl:NamedIndividual>
    


    <!-- http://purl.obolibrary.org/obo/GAZ_00068074 -->

    <owl:NamedIndividual rdf:about="http://purl.obolibrary.org/obo/GAZ_00068074">
        <rdf:type rdf:resource="http://purl.obolibrary.org/obo/ENVO_00000856"/>
        <obo:RO_0001025 rdf:resource="http://purl.obolibrary.org/obo/GAZ_00000439"/>
        <obo:IAO_0000115>A municipality in the Chimaltenango Department of Guatemala.</obo:IAO_0000115>
        <oboInOwl:hasOBONamespace>GAZ</oboInOwl:hasOBONamespace>
        <oboInOwl:id>GAZ:00068074</oboInOwl:id>
        <rdfs:label>Municipality of San Jose Poaquil</rdfs:label>
    </owl:NamedIndividual>
    


    <!-- http://purl.obolibrary.org/obo/GAZ_00068075 -->

    <owl:NamedIndividual rdf:about="http://purl.obolibrary.org/obo/GAZ_00068075">
        <rdf:type rdf:resource="http://purl.obolibrary.org/obo/ENVO_00000856"/>
        <obo:RO_0001025 rdf:resource="http://purl.obolibrary.org/obo/GAZ_00000439"/>
        <obo:IAO_0000115>A municipality in the Chimaltenango Department of Guatemala.</obo:IAO_0000115>
        <oboInOwl:hasOBONamespace>GAZ</oboInOwl:hasOBONamespace>
        <oboInOwl:id>GAZ:00068075</oboInOwl:id>
        <rdfs:label>Municipality of San Martin Jilotepeque</rdfs:label>
    </owl:NamedIndividual>
    


    <!-- http://purl.obolibrary.org/obo/GAZ_00068076 -->

    <owl:NamedIndividual rdf:about="http://purl.obolibrary.org/obo/GAZ_00068076">
        <rdf:type rdf:resource="http://purl.obolibrary.org/obo/ENVO_00000856"/>
        <obo:RO_0001025 rdf:resource="http://purl.obolibrary.org/obo/GAZ_00000439"/>
        <obo:IAO_0000115>A municipality in the Chimaltenango Department of Guatemala.</obo:IAO_0000115>
        <oboInOwl:hasOBONamespace>GAZ</oboInOwl:hasOBONamespace>
        <oboInOwl:id>GAZ:00068076</oboInOwl:id>
        <rdfs:label>Municipality of San Andres Itzapa</rdfs:label>
    </owl:NamedIndividual>
    


    <!-- http://purl.obolibrary.org/obo/GAZ_00068077 -->

    <owl:NamedIndividual rdf:about="http://purl.obolibrary.org/obo/GAZ_00068077">
        <rdf:type rdf:resource="http://purl.obolibrary.org/obo/ENVO_00000856"/>
        <obo:RO_0001025 rdf:resource="http://purl.obolibrary.org/obo/GAZ_00000439"/>
        <obo:IAO_0000115>A municipality in the Chimaltenango Department of Guatemala.</obo:IAO_0000115>
        <oboInOwl:hasOBONamespace>GAZ</oboInOwl:hasOBONamespace>
        <oboInOwl:id>GAZ:00068077</oboInOwl:id>
        <rdfs:label>Municipality of Santa Cruz Balanya</rdfs:label>
    </owl:NamedIndividual>
    


    <!-- http://purl.obolibrary.org/obo/GAZ_00068078 -->

    <owl:NamedIndividual rdf:about="http://purl.obolibrary.org/obo/GAZ_00068078">
        <rdf:type rdf:resource="http://purl.obolibrary.org/obo/ENVO_00000856"/>
        <obo:RO_0001025 rdf:resource="http://purl.obolibrary.org/obo/GAZ_00000439"/>
        <obo:IAO_0000115>A municipality in the Chimaltenango Department of Guatemala.</obo:IAO_0000115>
        <oboInOwl:hasOBONamespace>GAZ</oboInOwl:hasOBONamespace>
        <oboInOwl:id>GAZ:00068078</oboInOwl:id>
        <rdfs:label>Municipality of Pochuta</rdfs:label>
    </owl:NamedIndividual>
    


    <!-- http://purl.obolibrary.org/obo/GAZ_00068079 -->

    <owl:NamedIndividual rdf:about="http://purl.obolibrary.org/obo/GAZ_00068079">
        <rdf:type rdf:resource="http://purl.obolibrary.org/obo/ENVO_00000856"/>
        <obo:RO_0001025 rdf:resource="http://purl.obolibrary.org/obo/GAZ_00000439"/>
        <obo:IAO_0000115>A municipality in the Chimaltenango Department of Guatemala.</obo:IAO_0000115>
        <oboInOwl:hasOBONamespace>GAZ</oboInOwl:hasOBONamespace>
        <oboInOwl:id>GAZ:00068079</oboInOwl:id>
        <rdfs:label>Municipality of Yepocapa</rdfs:label>
    </owl:NamedIndividual>
    


    <!-- http://purl.obolibrary.org/obo/GAZ_00068080 -->

    <owl:NamedIndividual rdf:about="http://purl.obolibrary.org/obo/GAZ_00068080">
        <rdf:type rdf:resource="http://purl.obolibrary.org/obo/ENVO_00000856"/>
        <obo:RO_0001025 rdf:resource="http://purl.obolibrary.org/obo/GAZ_00000439"/>
        <obo:IAO_0000115>A municipality in the Chimaltenango Department of Guatemala.</obo:IAO_0000115>
        <oboInOwl:hasOBONamespace>GAZ</oboInOwl:hasOBONamespace>
        <oboInOwl:id>GAZ:00068080</oboInOwl:id>
        <rdfs:label>Municipality of Santa Apolonia</rdfs:label>
    </owl:NamedIndividual>
    


    <!-- http://purl.obolibrary.org/obo/GAZ_00068081 -->

    <owl:NamedIndividual rdf:about="http://purl.obolibrary.org/obo/GAZ_00068081">
        <rdf:type rdf:resource="http://purl.obolibrary.org/obo/ENVO_00000856"/>
        <obo:RO_0001025 rdf:resource="http://purl.obolibrary.org/obo/GAZ_00000446"/>
        <obo:IAO_0000115>A municipality in the Chiquimula Department of Guatemala.</obo:IAO_0000115>
        <oboInOwl:hasOBONamespace>GAZ</oboInOwl:hasOBONamespace>
        <oboInOwl:id>GAZ:00068081</oboInOwl:id>
        <rdfs:label>Municipality of Concepcion Las Minas</rdfs:label>
    </owl:NamedIndividual>
    


    <!-- http://purl.obolibrary.org/obo/GAZ_00068082 -->

    <owl:NamedIndividual rdf:about="http://purl.obolibrary.org/obo/GAZ_00068082">
        <obo:RO_0001025 rdf:resource="http://purl.obolibrary.org/obo/GAZ_00000439"/>
        <obo:IAO_0000115>A municipality in the Chimaltenango Department of Guatemala.</obo:IAO_0000115>
        <oboInOwl:hasOBONamespace>GAZ</oboInOwl:hasOBONamespace>
        <oboInOwl:id>GAZ:00068082</oboInOwl:id>
        <rdfs:label>Municipality of San Juan Comalapa</rdfs:label>
    </owl:NamedIndividual>
    


    <!-- http://purl.obolibrary.org/obo/GAZ_00068083 -->

    <owl:NamedIndividual rdf:about="http://purl.obolibrary.org/obo/GAZ_00068083">
        <rdf:type rdf:resource="http://purl.obolibrary.org/obo/ENVO_00000856"/>
        <obo:RO_0001025 rdf:resource="http://purl.obolibrary.org/obo/GAZ_00000439"/>
        <obo:IAO_0000115>A municipality in the Chimaltenango Department of Guatemala.</obo:IAO_0000115>
        <oboInOwl:hasOBONamespace>GAZ</oboInOwl:hasOBONamespace>
        <oboInOwl:id>GAZ:00068083</oboInOwl:id>
        <rdfs:label>Municipality of Acatenango</rdfs:label>
    </owl:NamedIndividual>
    


    <!-- http://purl.obolibrary.org/obo/GAZ_00068084 -->

    <owl:NamedIndividual rdf:about="http://purl.obolibrary.org/obo/GAZ_00068084">
        <rdf:type rdf:resource="http://purl.obolibrary.org/obo/ENVO_00000856"/>
        <obo:RO_0001025 rdf:resource="http://purl.obolibrary.org/obo/GAZ_00000439"/>
        <obo:IAO_0000115>A municipality in the Chimaltenango Department of Guatemala.</obo:IAO_0000115>
        <oboInOwl:hasOBONamespace>GAZ</oboInOwl:hasOBONamespace>
        <oboInOwl:id>GAZ:00068084</oboInOwl:id>
        <rdfs:label>Municipality of El Tejar</rdfs:label>
    </owl:NamedIndividual>
    


    <!-- http://purl.obolibrary.org/obo/GAZ_00068085 -->

    <owl:NamedIndividual rdf:about="http://purl.obolibrary.org/obo/GAZ_00068085">
        <rdf:type rdf:resource="http://purl.obolibrary.org/obo/ENVO_00000856"/>
        <obo:RO_0001025 rdf:resource="http://purl.obolibrary.org/obo/GAZ_00000439"/>
        <obo:IAO_0000115>A municipality in the Chimaltenango Department of Guatemala.</obo:IAO_0000115>
        <oboInOwl:hasOBONamespace>GAZ</oboInOwl:hasOBONamespace>
        <oboInOwl:id>GAZ:00068085</oboInOwl:id>
        <rdfs:label>Municipality of Chimaltenango</rdfs:label>
    </owl:NamedIndividual>
    


    <!-- http://purl.obolibrary.org/obo/GAZ_00068086 -->

    <owl:NamedIndividual rdf:about="http://purl.obolibrary.org/obo/GAZ_00068086">
        <rdf:type rdf:resource="http://purl.obolibrary.org/obo/ENVO_00000856"/>
        <obo:RO_0001025 rdf:resource="http://purl.obolibrary.org/obo/GAZ_00000446"/>
        <obo:IAO_0000115>A municipality in the Chiquimula Department of Guatemala.</obo:IAO_0000115>
        <oboInOwl:hasOBONamespace>GAZ</oboInOwl:hasOBONamespace>
        <oboInOwl:id>GAZ:00068086</oboInOwl:id>
        <rdfs:label>Municipality of Camotan</rdfs:label>
    </owl:NamedIndividual>
    


    <!-- http://purl.obolibrary.org/obo/GAZ_00068087 -->

    <owl:NamedIndividual rdf:about="http://purl.obolibrary.org/obo/GAZ_00068087">
        <rdf:type rdf:resource="http://purl.obolibrary.org/obo/ENVO_00000856"/>
        <obo:RO_0001025 rdf:resource="http://purl.obolibrary.org/obo/GAZ_00000446"/>
        <obo:IAO_0000115>A municipality in the Chiquimula Department of Guatemala.</obo:IAO_0000115>
        <oboInOwl:hasOBONamespace>GAZ</oboInOwl:hasOBONamespace>
        <oboInOwl:id>GAZ:00068087</oboInOwl:id>
        <rdfs:label>Municipality of Chiquimula</rdfs:label>
    </owl:NamedIndividual>
    


    <!-- http://purl.obolibrary.org/obo/GAZ_00068088 -->

    <owl:NamedIndividual rdf:about="http://purl.obolibrary.org/obo/GAZ_00068088">
        <rdf:type rdf:resource="http://purl.obolibrary.org/obo/ENVO_00000856"/>
        <obo:RO_0001025 rdf:resource="http://purl.obolibrary.org/obo/GAZ_00000446"/>
        <obo:IAO_0000115>A municipality in the Chiquimula Department of Guatemala.</obo:IAO_0000115>
        <oboInOwl:hasOBONamespace>GAZ</oboInOwl:hasOBONamespace>
        <oboInOwl:id>GAZ:00068088</oboInOwl:id>
        <rdfs:label>Municipality of Esquipulas</rdfs:label>
    </owl:NamedIndividual>
    


    <!-- http://purl.obolibrary.org/obo/GAZ_00068089 -->

    <owl:NamedIndividual rdf:about="http://purl.obolibrary.org/obo/GAZ_00068089">
        <rdf:type rdf:resource="http://purl.obolibrary.org/obo/ENVO_00000856"/>
        <obo:RO_0001025 rdf:resource="http://purl.obolibrary.org/obo/GAZ_00000446"/>
        <obo:IAO_0000115>A municipality in the Chiquimula Department of Guatemala.</obo:IAO_0000115>
        <oboInOwl:hasOBONamespace>GAZ</oboInOwl:hasOBONamespace>
        <oboInOwl:id>GAZ:00068089</oboInOwl:id>
        <rdfs:label>Municipality of Olopa</rdfs:label>
    </owl:NamedIndividual>
    


    <!-- http://purl.obolibrary.org/obo/GAZ_00068090 -->

    <owl:NamedIndividual rdf:about="http://purl.obolibrary.org/obo/GAZ_00068090">
        <rdf:type rdf:resource="http://purl.obolibrary.org/obo/ENVO_00000856"/>
        <obo:RO_0001025 rdf:resource="http://purl.obolibrary.org/obo/GAZ_00000446"/>
        <obo:IAO_0000115>A municipality in the Chiquimula Department of Guatemala.</obo:IAO_0000115>
        <oboInOwl:hasOBONamespace>GAZ</oboInOwl:hasOBONamespace>
        <oboInOwl:id>GAZ:00068090</oboInOwl:id>
        <rdfs:label>Municipality of San Jacinto</rdfs:label>
    </owl:NamedIndividual>
    


    <!-- http://purl.obolibrary.org/obo/GAZ_00068091 -->

    <owl:NamedIndividual rdf:about="http://purl.obolibrary.org/obo/GAZ_00068091">
        <rdf:type rdf:resource="http://purl.obolibrary.org/obo/ENVO_00000856"/>
        <obo:RO_0001025 rdf:resource="http://purl.obolibrary.org/obo/GAZ_00000446"/>
        <obo:IAO_0000115>A municipality in the Chiquimula Department of Guatemala.</obo:IAO_0000115>
        <oboInOwl:hasOBONamespace>GAZ</oboInOwl:hasOBONamespace>
        <oboInOwl:id>GAZ:00068091</oboInOwl:id>
        <rdfs:label>Municipality of San Juan La Ermita</rdfs:label>
    </owl:NamedIndividual>
    


    <!-- http://purl.obolibrary.org/obo/GAZ_00068092 -->

    <owl:NamedIndividual rdf:about="http://purl.obolibrary.org/obo/GAZ_00068092">
        <rdf:type rdf:resource="http://purl.obolibrary.org/obo/ENVO_00000856"/>
        <obo:RO_0001025 rdf:resource="http://purl.obolibrary.org/obo/GAZ_00000446"/>
        <obo:IAO_0000115>A municipality in the Chiquimula Department of Guatemala.</obo:IAO_0000115>
        <oboInOwl:hasOBONamespace>GAZ</oboInOwl:hasOBONamespace>
        <oboInOwl:id>GAZ:00068092</oboInOwl:id>
        <rdfs:label>Municipality of San Jose La Arada</rdfs:label>
    </owl:NamedIndividual>
    


    <!-- http://purl.obolibrary.org/obo/GAZ_00068093 -->

    <owl:NamedIndividual rdf:about="http://purl.obolibrary.org/obo/GAZ_00068093">
        <rdf:type rdf:resource="http://purl.obolibrary.org/obo/ENVO_00000856"/>
        <obo:RO_0001025 rdf:resource="http://purl.obolibrary.org/obo/GAZ_00000446"/>
        <obo:IAO_0000115>A municipality in the Chiquimula Department of Guatemala.</obo:IAO_0000115>
        <oboInOwl:hasOBONamespace>GAZ</oboInOwl:hasOBONamespace>
        <oboInOwl:id>GAZ:00068093</oboInOwl:id>
        <rdfs:label>Municipality of Quezaltepeque</rdfs:label>
    </owl:NamedIndividual>
    


    <!-- http://purl.obolibrary.org/obo/GAZ_00068094 -->

    <owl:NamedIndividual rdf:about="http://purl.obolibrary.org/obo/GAZ_00068094">
        <rdf:type rdf:resource="http://purl.obolibrary.org/obo/ENVO_00000856"/>
        <obo:RO_0001025 rdf:resource="http://purl.obolibrary.org/obo/GAZ_00000446"/>
        <obo:IAO_0000115>A municipality in the Chiquimula Department of Guatemala.</obo:IAO_0000115>
        <oboInOwl:hasOBONamespace>GAZ</oboInOwl:hasOBONamespace>
        <oboInOwl:id>GAZ:00068094</oboInOwl:id>
        <rdfs:label>Municipality of Jocotan</rdfs:label>
    </owl:NamedIndividual>
    


    <!-- http://purl.obolibrary.org/obo/GAZ_00068095 -->

    <owl:NamedIndividual rdf:about="http://purl.obolibrary.org/obo/GAZ_00068095">
        <rdf:type rdf:resource="http://purl.obolibrary.org/obo/ENVO_00000856"/>
        <obo:RO_0001025 rdf:resource="http://purl.obolibrary.org/obo/GAZ_00000476"/>
        <obo:IAO_0000115>A municipality in the El Progreso Department of Guatemala.</obo:IAO_0000115>
        <oboInOwl:hasOBONamespace>GAZ</oboInOwl:hasOBONamespace>
        <oboInOwl:id>GAZ:00068095</oboInOwl:id>
        <rdfs:label>Municipality of Sansare</rdfs:label>
    </owl:NamedIndividual>
    


    <!-- http://purl.obolibrary.org/obo/GAZ_00068096 -->

    <owl:NamedIndividual rdf:about="http://purl.obolibrary.org/obo/GAZ_00068096">
        <rdf:type rdf:resource="http://purl.obolibrary.org/obo/ENVO_00000856"/>
        <obo:RO_0001025 rdf:resource="http://purl.obolibrary.org/obo/GAZ_00000476"/>
        <obo:IAO_0000115>A municipality in the El Progreso Department of Guatemala.</obo:IAO_0000115>
        <oboInOwl:hasOBONamespace>GAZ</oboInOwl:hasOBONamespace>
        <oboInOwl:id>GAZ:00068096</oboInOwl:id>
        <rdfs:label>Municipality of Morazan</rdfs:label>
    </owl:NamedIndividual>
    


    <!-- http://purl.obolibrary.org/obo/GAZ_00068097 -->

    <owl:NamedIndividual rdf:about="http://purl.obolibrary.org/obo/GAZ_00068097">
        <rdf:type rdf:resource="http://purl.obolibrary.org/obo/ENVO_00000856"/>
        <obo:RO_0001025 rdf:resource="http://purl.obolibrary.org/obo/GAZ_00000476"/>
        <obo:IAO_0000115>A municipality in the El Progreso Department of Guatemala.</obo:IAO_0000115>
        <oboInOwl:hasOBONamespace>GAZ</oboInOwl:hasOBONamespace>
        <oboInOwl:id>GAZ:00068097</oboInOwl:id>
        <rdfs:label>Municipality of San Cristobal Acasaguastlan</rdfs:label>
    </owl:NamedIndividual>
    


    <!-- http://purl.obolibrary.org/obo/GAZ_00068098 -->

    <owl:NamedIndividual rdf:about="http://purl.obolibrary.org/obo/GAZ_00068098">
        <rdf:type rdf:resource="http://purl.obolibrary.org/obo/ENVO_00000856"/>
        <obo:RO_0001025 rdf:resource="http://purl.obolibrary.org/obo/GAZ_00000476"/>
        <obo:IAO_0000115>A municipality in the El Progreso Department of Guatemala.</obo:IAO_0000115>
        <oboInOwl:hasOBONamespace>GAZ</oboInOwl:hasOBONamespace>
        <oboInOwl:id>GAZ:00068098</oboInOwl:id>
        <rdfs:label>Municipality of El Jicaro</rdfs:label>
    </owl:NamedIndividual>
    


    <!-- http://purl.obolibrary.org/obo/GAZ_00068099 -->

    <owl:NamedIndividual rdf:about="http://purl.obolibrary.org/obo/GAZ_00068099">
        <rdf:type rdf:resource="http://purl.obolibrary.org/obo/ENVO_00000856"/>
        <obo:RO_0001025 rdf:resource="http://purl.obolibrary.org/obo/GAZ_00000476"/>
        <obo:IAO_0000115>A municipality in the El Progreso Department of Guatemala.</obo:IAO_0000115>
        <oboInOwl:hasOBONamespace>GAZ</oboInOwl:hasOBONamespace>
        <oboInOwl:id>GAZ:00068099</oboInOwl:id>
        <rdfs:label>Municipality of San Antonio La Paz</rdfs:label>
    </owl:NamedIndividual>
    


    <!-- http://purl.obolibrary.org/obo/GAZ_00068100 -->

    <owl:NamedIndividual rdf:about="http://purl.obolibrary.org/obo/GAZ_00068100">
        <rdf:type rdf:resource="http://purl.obolibrary.org/obo/ENVO_00000856"/>
        <obo:RO_0001025 rdf:resource="http://purl.obolibrary.org/obo/GAZ_00000476"/>
        <obo:IAO_0000115>A municipality in the El Progreso Department of Guatemala.</obo:IAO_0000115>
        <oboInOwl:hasOBONamespace>GAZ</oboInOwl:hasOBONamespace>
        <oboInOwl:id>GAZ:00068100</oboInOwl:id>
        <rdfs:label>Municipality of Guastatoya</rdfs:label>
    </owl:NamedIndividual>
    


    <!-- http://purl.obolibrary.org/obo/GAZ_00068101 -->

    <owl:NamedIndividual rdf:about="http://purl.obolibrary.org/obo/GAZ_00068101">
        <rdf:type rdf:resource="http://purl.obolibrary.org/obo/ENVO_00000856"/>
        <obo:RO_0001025 rdf:resource="http://purl.obolibrary.org/obo/GAZ_00000476"/>
        <obo:IAO_0000115>A municipality in the El Progreso Department of Guatemala.</obo:IAO_0000115>
        <oboInOwl:hasOBONamespace>GAZ</oboInOwl:hasOBONamespace>
        <oboInOwl:id>GAZ:00068101</oboInOwl:id>
        <rdfs:label>Municipality of San Agustin Acasaguastlan</rdfs:label>
    </owl:NamedIndividual>
    


    <!-- http://purl.obolibrary.org/obo/GAZ_00068102 -->

    <owl:NamedIndividual rdf:about="http://purl.obolibrary.org/obo/GAZ_00068102">
        <rdf:type rdf:resource="http://purl.obolibrary.org/obo/ENVO_00000856"/>
        <obo:RO_0001025 rdf:resource="http://purl.obolibrary.org/obo/GAZ_00000477"/>
        <obo:IAO_0000115>A municipality in the Escuintla Department of Guatemala.</obo:IAO_0000115>
        <oboInOwl:hasOBONamespace>GAZ</oboInOwl:hasOBONamespace>
        <oboInOwl:id>GAZ:00068102</oboInOwl:id>
        <rdfs:label>Municipality of San Jose</rdfs:label>
    </owl:NamedIndividual>
    


    <!-- http://purl.obolibrary.org/obo/GAZ_00068103 -->

    <owl:NamedIndividual rdf:about="http://purl.obolibrary.org/obo/GAZ_00068103">
        <rdf:type rdf:resource="http://purl.obolibrary.org/obo/ENVO_00000856"/>
        <obo:RO_0001025 rdf:resource="http://purl.obolibrary.org/obo/GAZ_00000477"/>
        <obo:IAO_0000115>A municipality in the Escuintla Department of Guatemala.</obo:IAO_0000115>
        <oboInOwl:hasOBONamespace>GAZ</oboInOwl:hasOBONamespace>
        <oboInOwl:id>GAZ:00068103</oboInOwl:id>
        <rdfs:label>Municipality of Nueva Concepcion</rdfs:label>
    </owl:NamedIndividual>
    


    <!-- http://purl.obolibrary.org/obo/GAZ_00068104 -->

    <owl:NamedIndividual rdf:about="http://purl.obolibrary.org/obo/GAZ_00068104">
        <rdf:type rdf:resource="http://purl.obolibrary.org/obo/ENVO_00000856"/>
        <obo:RO_0001025 rdf:resource="http://purl.obolibrary.org/obo/GAZ_00000477"/>
        <obo:IAO_0000115>A municipality in the Escuintla Department of Guatemala.</obo:IAO_0000115>
        <oboInOwl:hasOBONamespace>GAZ</oboInOwl:hasOBONamespace>
        <oboInOwl:id>GAZ:00068104</oboInOwl:id>
        <rdfs:label>Municipality of Tiquisate</rdfs:label>
    </owl:NamedIndividual>
    


    <!-- http://purl.obolibrary.org/obo/GAZ_00068105 -->

    <owl:NamedIndividual rdf:about="http://purl.obolibrary.org/obo/GAZ_00068105">
        <rdf:type rdf:resource="http://purl.obolibrary.org/obo/ENVO_00000856"/>
        <obo:RO_0001025 rdf:resource="http://purl.obolibrary.org/obo/GAZ_00000477"/>
        <obo:IAO_0000115>A municipality in the Escuintla Department of Guatemala.</obo:IAO_0000115>
        <oboInOwl:hasOBONamespace>GAZ</oboInOwl:hasOBONamespace>
        <oboInOwl:id>GAZ:00068105</oboInOwl:id>
        <rdfs:label>Municipality of San Vicente Pacaya</rdfs:label>
    </owl:NamedIndividual>
    


    <!-- http://purl.obolibrary.org/obo/GAZ_00068106 -->

    <owl:NamedIndividual rdf:about="http://purl.obolibrary.org/obo/GAZ_00068106">
        <rdf:type rdf:resource="http://purl.obolibrary.org/obo/ENVO_00000856"/>
        <obo:RO_0001025 rdf:resource="http://purl.obolibrary.org/obo/GAZ_00000477"/>
        <obo:IAO_0000115>A municipality in the Escuintla Department of Guatemala.</obo:IAO_0000115>
        <oboInOwl:hasOBONamespace>GAZ</oboInOwl:hasOBONamespace>
        <oboInOwl:id>GAZ:00068106</oboInOwl:id>
        <rdfs:label>Municipality of La Gomera</rdfs:label>
    </owl:NamedIndividual>
    


    <!-- http://purl.obolibrary.org/obo/GAZ_00068107 -->

    <owl:NamedIndividual rdf:about="http://purl.obolibrary.org/obo/GAZ_00068107">
        <rdf:type rdf:resource="http://purl.obolibrary.org/obo/ENVO_00000856"/>
        <obo:RO_0001025 rdf:resource="http://purl.obolibrary.org/obo/GAZ_00000477"/>
        <obo:IAO_0000115>A municipality in the Escuintla Department of Guatemala.</obo:IAO_0000115>
        <oboInOwl:hasOBONamespace>GAZ</oboInOwl:hasOBONamespace>
        <oboInOwl:id>GAZ:00068107</oboInOwl:id>
        <rdfs:label>Municipality of Santa Lucia Cotzumalguapa</rdfs:label>
    </owl:NamedIndividual>
    


    <!-- http://purl.obolibrary.org/obo/GAZ_00068108 -->

    <owl:NamedIndividual rdf:about="http://purl.obolibrary.org/obo/GAZ_00068108">
        <rdf:type rdf:resource="http://purl.obolibrary.org/obo/ENVO_00000856"/>
        <obo:RO_0001025 rdf:resource="http://purl.obolibrary.org/obo/GAZ_00000477"/>
        <obo:IAO_0000115>A municipality in the Escuintla Department of Guatemala.</obo:IAO_0000115>
        <oboInOwl:hasOBONamespace>GAZ</oboInOwl:hasOBONamespace>
        <oboInOwl:id>GAZ:00068108</oboInOwl:id>
        <rdfs:label>Municipality of Iztapa</rdfs:label>
    </owl:NamedIndividual>
    


    <!-- http://purl.obolibrary.org/obo/GAZ_00068109 -->

    <owl:NamedIndividual rdf:about="http://purl.obolibrary.org/obo/GAZ_00068109">
        <rdf:type rdf:resource="http://purl.obolibrary.org/obo/ENVO_00000856"/>
        <obo:RO_0001025 rdf:resource="http://purl.obolibrary.org/obo/GAZ_00000477"/>
        <obo:IAO_0000115>A municipality in the Escuintla Department of Guatemala.</obo:IAO_0000115>
        <oboInOwl:hasOBONamespace>GAZ</oboInOwl:hasOBONamespace>
        <oboInOwl:id>GAZ:00068109</oboInOwl:id>
        <rdfs:label>Municipality of Siquinala</rdfs:label>
    </owl:NamedIndividual>
    


    <!-- http://purl.obolibrary.org/obo/GAZ_00068110 -->

    <owl:NamedIndividual rdf:about="http://purl.obolibrary.org/obo/GAZ_00068110">
        <rdf:type rdf:resource="http://purl.obolibrary.org/obo/ENVO_00000856"/>
        <obo:RO_0001025 rdf:resource="http://purl.obolibrary.org/obo/GAZ_00000477"/>
        <obo:IAO_0000115>A municipality in the Escuintla Department of Guatemala.</obo:IAO_0000115>
        <oboInOwl:hasOBONamespace>GAZ</oboInOwl:hasOBONamespace>
        <oboInOwl:id>GAZ:00068110</oboInOwl:id>
        <rdfs:label>Municipality of Guanagazapa</rdfs:label>
    </owl:NamedIndividual>
    


    <!-- http://purl.obolibrary.org/obo/GAZ_00068111 -->

    <owl:NamedIndividual rdf:about="http://purl.obolibrary.org/obo/GAZ_00068111">
        <rdf:type rdf:resource="http://purl.obolibrary.org/obo/ENVO_00000856"/>
        <obo:RO_0001025 rdf:resource="http://purl.obolibrary.org/obo/GAZ_00000477"/>
        <obo:IAO_0000115>A municipality in the Escuintla Department of Guatemala.</obo:IAO_0000115>
        <oboInOwl:hasOBONamespace>GAZ</oboInOwl:hasOBONamespace>
        <oboInOwl:id>GAZ:00068111</oboInOwl:id>
        <rdfs:label>Municipality of Escuintla</rdfs:label>
    </owl:NamedIndividual>
    


    <!-- http://purl.obolibrary.org/obo/GAZ_00068112 -->

    <owl:NamedIndividual rdf:about="http://purl.obolibrary.org/obo/GAZ_00068112">
        <rdf:type rdf:resource="http://purl.obolibrary.org/obo/ENVO_00000856"/>
        <obo:RO_0001025 rdf:resource="http://purl.obolibrary.org/obo/GAZ_00000477"/>
        <obo:IAO_0000115>A municipality in the Escuintla Department of Guatemala.</obo:IAO_0000115>
        <oboInOwl:hasOBONamespace>GAZ</oboInOwl:hasOBONamespace>
        <oboInOwl:id>GAZ:00068112</oboInOwl:id>
        <rdfs:label>Municipality of Masagua</rdfs:label>
    </owl:NamedIndividual>
    


    <!-- http://purl.obolibrary.org/obo/GAZ_00068113 -->

    <owl:NamedIndividual rdf:about="http://purl.obolibrary.org/obo/GAZ_00068113">
        <rdf:type rdf:resource="http://purl.obolibrary.org/obo/ENVO_00000856"/>
        <obo:RO_0001025 rdf:resource="http://purl.obolibrary.org/obo/GAZ_00000477"/>
        <obo:IAO_0000115>A municipality in the Escuintla Department of Guatemala.</obo:IAO_0000115>
        <oboInOwl:hasOBONamespace>GAZ</oboInOwl:hasOBONamespace>
        <oboInOwl:id>GAZ:00068113</oboInOwl:id>
        <rdfs:label>Municipality of Palin</rdfs:label>
    </owl:NamedIndividual>
    


    <!-- http://purl.obolibrary.org/obo/GAZ_00068114 -->

    <owl:NamedIndividual rdf:about="http://purl.obolibrary.org/obo/GAZ_00068114">
        <rdf:type rdf:resource="http://purl.obolibrary.org/obo/ENVO_00000856"/>
        <obo:RO_0001025 rdf:resource="http://purl.obolibrary.org/obo/GAZ_00000477"/>
        <obo:IAO_0000115>A municipality in the Escuintla Department of Guatemala.</obo:IAO_0000115>
        <oboInOwl:hasOBONamespace>GAZ</oboInOwl:hasOBONamespace>
        <oboInOwl:id>GAZ:00068114</oboInOwl:id>
        <rdfs:label>Municipality of La Democracia</rdfs:label>
    </owl:NamedIndividual>
    


    <!-- http://purl.obolibrary.org/obo/GAZ_00068115 -->

    <owl:NamedIndividual rdf:about="http://purl.obolibrary.org/obo/GAZ_00068115">
        <rdf:type rdf:resource="http://purl.obolibrary.org/obo/ENVO_00000856"/>
        <obo:RO_0001025 rdf:resource="http://purl.obolibrary.org/obo/GAZ_00005155"/>
        <obo:IAO_0000115>A municipality in the Guatemala Department of Guatemala.</obo:IAO_0000115>
        <oboInOwl:hasOBONamespace>GAZ</oboInOwl:hasOBONamespace>
        <oboInOwl:id>GAZ:00068115</oboInOwl:id>
        <rdfs:label>Municipality of Amatitlan</rdfs:label>
    </owl:NamedIndividual>
    


    <!-- http://purl.obolibrary.org/obo/GAZ_00068116 -->

    <owl:NamedIndividual rdf:about="http://purl.obolibrary.org/obo/GAZ_00068116">
        <rdf:type rdf:resource="http://purl.obolibrary.org/obo/ENVO_00000856"/>
        <obo:RO_0001025 rdf:resource="http://purl.obolibrary.org/obo/GAZ_00005155"/>
        <obo:IAO_0000115>A municipality in the Guatemala Department of Guatemala.</obo:IAO_0000115>
        <oboInOwl:hasOBONamespace>GAZ</oboInOwl:hasOBONamespace>
        <oboInOwl:id>GAZ:00068116</oboInOwl:id>
        <rdfs:label>Municipality of Chuarrancho</rdfs:label>
    </owl:NamedIndividual>
    


    <!-- http://purl.obolibrary.org/obo/GAZ_00068117 -->

    <owl:NamedIndividual rdf:about="http://purl.obolibrary.org/obo/GAZ_00068117">
        <rdf:type rdf:resource="http://purl.obolibrary.org/obo/ENVO_00000856"/>
        <obo:RO_0001025 rdf:resource="http://purl.obolibrary.org/obo/GAZ_00005155"/>
        <obo:IAO_0000115>A municipality in the Guatemala Department of Guatemala.</obo:IAO_0000115>
        <oboInOwl:hasOBONamespace>GAZ</oboInOwl:hasOBONamespace>
        <oboInOwl:id>GAZ:00068117</oboInOwl:id>
        <rdfs:label>Municipality of San Pedro Sacatepequez</rdfs:label>
    </owl:NamedIndividual>
    


    <!-- http://purl.obolibrary.org/obo/GAZ_00068118 -->

    <owl:NamedIndividual rdf:about="http://purl.obolibrary.org/obo/GAZ_00068118">
        <rdf:type rdf:resource="http://purl.obolibrary.org/obo/ENVO_00000856"/>
        <obo:RO_0001025 rdf:resource="http://purl.obolibrary.org/obo/GAZ_00005155"/>
        <obo:IAO_0000115>A municipality in the Guatemala Department of Guatemala.</obo:IAO_0000115>
        <oboInOwl:hasOBONamespace>GAZ</oboInOwl:hasOBONamespace>
        <oboInOwl:id>GAZ:00068118</oboInOwl:id>
        <rdfs:label>Municipality of Fraijanes</rdfs:label>
    </owl:NamedIndividual>
    


    <!-- http://purl.obolibrary.org/obo/GAZ_00068119 -->

    <owl:NamedIndividual rdf:about="http://purl.obolibrary.org/obo/GAZ_00068119">
        <rdf:type rdf:resource="http://purl.obolibrary.org/obo/ENVO_00000856"/>
        <obo:RO_0001025 rdf:resource="http://purl.obolibrary.org/obo/GAZ_00005155"/>
        <obo:IAO_0000115>A municipality in the Guatemala Department of Guatemala.</obo:IAO_0000115>
        <oboInOwl:hasOBONamespace>GAZ</oboInOwl:hasOBONamespace>
        <oboInOwl:id>GAZ:00068119</oboInOwl:id>
        <rdfs:label>Municipality of Petapa</rdfs:label>
    </owl:NamedIndividual>
    


    <!-- http://purl.obolibrary.org/obo/GAZ_00068120 -->

    <owl:NamedIndividual rdf:about="http://purl.obolibrary.org/obo/GAZ_00068120">
        <rdf:type rdf:resource="http://purl.obolibrary.org/obo/ENVO_00000856"/>
        <obo:RO_0001025 rdf:resource="http://purl.obolibrary.org/obo/GAZ_00005155"/>
        <obo:IAO_0000115>A municipality in the Guatemala Department of Guatemala.</obo:IAO_0000115>
        <oboInOwl:hasOBONamespace>GAZ</oboInOwl:hasOBONamespace>
        <oboInOwl:id>GAZ:00068120</oboInOwl:id>
        <rdfs:label>Municipality of Chinautla</rdfs:label>
    </owl:NamedIndividual>
    


    <!-- http://purl.obolibrary.org/obo/GAZ_00068121 -->

    <owl:NamedIndividual rdf:about="http://purl.obolibrary.org/obo/GAZ_00068121">
        <rdf:type rdf:resource="http://purl.obolibrary.org/obo/ENVO_00000856"/>
        <obo:RO_0001025 rdf:resource="http://purl.obolibrary.org/obo/GAZ_00005155"/>
        <obo:IAO_0000115>A municipality in the Guatemala Department of Guatemala.</obo:IAO_0000115>
        <oboInOwl:hasOBONamespace>GAZ</oboInOwl:hasOBONamespace>
        <oboInOwl:id>GAZ:00068121</oboInOwl:id>
        <rdfs:label>Municipality of Villa Nueva</rdfs:label>
    </owl:NamedIndividual>
    


    <!-- http://purl.obolibrary.org/obo/GAZ_00068122 -->

    <owl:NamedIndividual rdf:about="http://purl.obolibrary.org/obo/GAZ_00068122">
        <rdf:type rdf:resource="http://purl.obolibrary.org/obo/ENVO_00000856"/>
        <obo:RO_0001025 rdf:resource="http://purl.obolibrary.org/obo/GAZ_00005155"/>
        <obo:IAO_0000115>A municipality in the Guatemala Department of Guatemala.</obo:IAO_0000115>
        <oboInOwl:hasOBONamespace>GAZ</oboInOwl:hasOBONamespace>
        <oboInOwl:id>GAZ:00068122</oboInOwl:id>
        <rdfs:label>Municipality of San Pedro Ayampuc</rdfs:label>
    </owl:NamedIndividual>
    


    <!-- http://purl.obolibrary.org/obo/GAZ_00068123 -->

    <owl:NamedIndividual rdf:about="http://purl.obolibrary.org/obo/GAZ_00068123">
        <rdf:type rdf:resource="http://purl.obolibrary.org/obo/ENVO_00000856"/>
        <obo:RO_0001025 rdf:resource="http://purl.obolibrary.org/obo/GAZ_00005155"/>
        <obo:IAO_0000115>A municipality in the Guatemala Department of Guatemala.</obo:IAO_0000115>
        <oboInOwl:hasOBONamespace>GAZ</oboInOwl:hasOBONamespace>
        <oboInOwl:id>GAZ:00068123</oboInOwl:id>
        <rdfs:label>Municipality of Santa Catarina Pinula</rdfs:label>
    </owl:NamedIndividual>
    


    <!-- http://purl.obolibrary.org/obo/GAZ_00068124 -->

    <owl:NamedIndividual rdf:about="http://purl.obolibrary.org/obo/GAZ_00068124">
        <rdf:type rdf:resource="http://purl.obolibrary.org/obo/ENVO_00000856"/>
        <obo:RO_0001025 rdf:resource="http://purl.obolibrary.org/obo/GAZ_00005155"/>
        <obo:IAO_0000115>A municipality in the Guatemala Department of Guatemala.</obo:IAO_0000115>
        <oboInOwl:hasOBONamespace>GAZ</oboInOwl:hasOBONamespace>
        <oboInOwl:id>GAZ:00068124</oboInOwl:id>
        <rdfs:label>Municipality of San Jose del Golfo</rdfs:label>
    </owl:NamedIndividual>
    


    <!-- http://purl.obolibrary.org/obo/GAZ_00068125 -->

    <owl:NamedIndividual rdf:about="http://purl.obolibrary.org/obo/GAZ_00068125">
        <rdf:type rdf:resource="http://purl.obolibrary.org/obo/ENVO_00000856"/>
        <obo:RO_0001025 rdf:resource="http://purl.obolibrary.org/obo/GAZ_00005155"/>
        <obo:IAO_0000115>A municipality in the Guatemala Department of Guatemala.</obo:IAO_0000115>
        <oboInOwl:hasOBONamespace>GAZ</oboInOwl:hasOBONamespace>
        <oboInOwl:id>GAZ:00068125</oboInOwl:id>
        <rdfs:label>Municipality of San Jose Pinula</rdfs:label>
    </owl:NamedIndividual>
    


    <!-- http://purl.obolibrary.org/obo/GAZ_00068126 -->

    <owl:NamedIndividual rdf:about="http://purl.obolibrary.org/obo/GAZ_00068126">
        <rdf:type rdf:resource="http://purl.obolibrary.org/obo/ENVO_00000856"/>
        <obo:RO_0001025 rdf:resource="http://purl.obolibrary.org/obo/GAZ_00005155"/>
        <obo:IAO_0000115>A municipality in the Guatemala Department of Guatemala.</obo:IAO_0000115>
        <oboInOwl:hasOBONamespace>GAZ</oboInOwl:hasOBONamespace>
        <oboInOwl:id>GAZ:00068126</oboInOwl:id>
        <rdfs:label>Municipality of Villa Canales</rdfs:label>
    </owl:NamedIndividual>
    


    <!-- http://purl.obolibrary.org/obo/GAZ_00068127 -->

    <owl:NamedIndividual rdf:about="http://purl.obolibrary.org/obo/GAZ_00068127">
        <rdf:type rdf:resource="http://purl.obolibrary.org/obo/ENVO_00000856"/>
        <obo:RO_0001025 rdf:resource="http://purl.obolibrary.org/obo/GAZ_00000483"/>
        <obo:IAO_0000115>A municipality in the Guatemalan Department of Huehuetenango.</obo:IAO_0000115>
        <oboInOwl:hasOBONamespace>GAZ</oboInOwl:hasOBONamespace>
        <oboInOwl:id>GAZ:00068127</oboInOwl:id>
        <rdfs:label>Municipality of Aguacatan</rdfs:label>
    </owl:NamedIndividual>
    


    <!-- http://purl.obolibrary.org/obo/GAZ_00068128 -->

    <owl:NamedIndividual rdf:about="http://purl.obolibrary.org/obo/GAZ_00068128">
        <rdf:type rdf:resource="http://purl.obolibrary.org/obo/ENVO_00000856"/>
        <obo:RO_0001025 rdf:resource="http://purl.obolibrary.org/obo/GAZ_00000483"/>
        <obo:IAO_0000115>A municipality in the Guatemalan Department of Huehuetenango.</obo:IAO_0000115>
        <oboInOwl:hasOBONamespace>GAZ</oboInOwl:hasOBONamespace>
        <oboInOwl:id>GAZ:00068128</oboInOwl:id>
        <rdfs:label>Municipality of Huehuetenango</rdfs:label>
    </owl:NamedIndividual>
    


    <!-- http://purl.obolibrary.org/obo/GAZ_00068129 -->

    <owl:NamedIndividual rdf:about="http://purl.obolibrary.org/obo/GAZ_00068129">
        <rdf:type rdf:resource="http://purl.obolibrary.org/obo/ENVO_00000856"/>
        <obo:RO_0001025 rdf:resource="http://purl.obolibrary.org/obo/GAZ_00000483"/>
        <obo:IAO_0000115>A municipality in the Guatemalan Department of Huehuetenango.</obo:IAO_0000115>
        <oboInOwl:hasOBONamespace>GAZ</oboInOwl:hasOBONamespace>
        <oboInOwl:id>GAZ:00068129</oboInOwl:id>
        <rdfs:label>Municipality of Chiantla</rdfs:label>
    </owl:NamedIndividual>
    


    <!-- http://purl.obolibrary.org/obo/GAZ_00068130 -->

    <owl:NamedIndividual rdf:about="http://purl.obolibrary.org/obo/GAZ_00068130">
        <rdf:type rdf:resource="http://purl.obolibrary.org/obo/ENVO_00000856"/>
        <obo:RO_0001025 rdf:resource="http://purl.obolibrary.org/obo/GAZ_00000483"/>
        <obo:IAO_0000115>A municipality in the Guatemalan Department of Huehuetenango.</obo:IAO_0000115>
        <oboInOwl:hasOBONamespace>GAZ</oboInOwl:hasOBONamespace>
        <oboInOwl:id>GAZ:00068130</oboInOwl:id>
        <rdfs:label>Municipality of Cuilco</rdfs:label>
    </owl:NamedIndividual>
    


    <!-- http://purl.obolibrary.org/obo/GAZ_00068131 -->

    <owl:NamedIndividual rdf:about="http://purl.obolibrary.org/obo/GAZ_00068131">
        <rdf:type rdf:resource="http://purl.obolibrary.org/obo/ENVO_00000856"/>
        <obo:RO_0001025 rdf:resource="http://purl.obolibrary.org/obo/GAZ_00000483"/>
        <obo:IAO_0000115>A municipality in the Guatemalan Department of Huehuetenango.</obo:IAO_0000115>
        <oboInOwl:hasOBONamespace>GAZ</oboInOwl:hasOBONamespace>
        <oboInOwl:id>GAZ:00068131</oboInOwl:id>
        <rdfs:label>Municipality of Concepcion Huista</rdfs:label>
    </owl:NamedIndividual>
    


    <!-- http://purl.obolibrary.org/obo/GAZ_00068132 -->

    <owl:NamedIndividual rdf:about="http://purl.obolibrary.org/obo/GAZ_00068132">
        <rdf:type rdf:resource="http://purl.obolibrary.org/obo/ENVO_00000856"/>
        <obo:RO_0001025 rdf:resource="http://purl.obolibrary.org/obo/GAZ_00000483"/>
        <obo:IAO_0000115>A municipality in the Guatemalan Department of Huehuetenango.</obo:IAO_0000115>
        <oboInOwl:hasOBONamespace>GAZ</oboInOwl:hasOBONamespace>
        <oboInOwl:id>GAZ:00068132</oboInOwl:id>
        <rdfs:label>Municipality of San Ildefonso Ixtahuacan</rdfs:label>
    </owl:NamedIndividual>
    


    <!-- http://purl.obolibrary.org/obo/GAZ_00068133 -->

    <owl:NamedIndividual rdf:about="http://purl.obolibrary.org/obo/GAZ_00068133">
        <rdf:type rdf:resource="http://purl.obolibrary.org/obo/ENVO_00000856"/>
        <obo:RO_0001025 rdf:resource="http://purl.obolibrary.org/obo/GAZ_00000483"/>
        <obo:IAO_0000115>A municipality in the Guatemalan Department of Huehuetenango.</obo:IAO_0000115>
        <oboInOwl:hasOBONamespace>GAZ</oboInOwl:hasOBONamespace>
        <oboInOwl:id>GAZ:00068133</oboInOwl:id>
        <rdfs:label>Municipality of Santa Cruz Barillas</rdfs:label>
    </owl:NamedIndividual>
    


    <!-- http://purl.obolibrary.org/obo/GAZ_00068134 -->

    <owl:NamedIndividual rdf:about="http://purl.obolibrary.org/obo/GAZ_00068134">
        <rdf:type rdf:resource="http://purl.obolibrary.org/obo/ENVO_00000856"/>
        <obo:RO_0001025 rdf:resource="http://purl.obolibrary.org/obo/GAZ_00000483"/>
        <obo:IAO_0000115>A municipality in the Guatemalan Department of Huehuetenango.</obo:IAO_0000115>
        <oboInOwl:hasOBONamespace>GAZ</oboInOwl:hasOBONamespace>
        <oboInOwl:id>GAZ:00068134</oboInOwl:id>
        <rdfs:label>Municipality of La Democracia</rdfs:label>
    </owl:NamedIndividual>
    


    <!-- http://purl.obolibrary.org/obo/GAZ_00068135 -->

    <owl:NamedIndividual rdf:about="http://purl.obolibrary.org/obo/GAZ_00068135">
        <rdf:type rdf:resource="http://purl.obolibrary.org/obo/ENVO_00000856"/>
        <obo:RO_0001025 rdf:resource="http://purl.obolibrary.org/obo/GAZ_00000483"/>
        <obo:IAO_0000115>A municipality in the Guatemalan Department of Huehuetenango.</obo:IAO_0000115>
        <oboInOwl:hasOBONamespace>GAZ</oboInOwl:hasOBONamespace>
        <oboInOwl:id>GAZ:00068135</oboInOwl:id>
        <rdfs:label>Municipality of La Libertad</rdfs:label>
    </owl:NamedIndividual>
    


    <!-- http://purl.obolibrary.org/obo/GAZ_00068136 -->

    <owl:NamedIndividual rdf:about="http://purl.obolibrary.org/obo/GAZ_00068136">
        <rdf:type rdf:resource="http://purl.obolibrary.org/obo/ENVO_00000856"/>
        <obo:RO_0001025 rdf:resource="http://purl.obolibrary.org/obo/GAZ_00000483"/>
        <obo:IAO_0000115>A municipality in the Guatemalan Department of Huehuetenango.</obo:IAO_0000115>
        <oboInOwl:hasOBONamespace>GAZ</oboInOwl:hasOBONamespace>
        <oboInOwl:id>GAZ:00068136</oboInOwl:id>
        <rdfs:label>Municipality of Nenton</rdfs:label>
    </owl:NamedIndividual>
    


    <!-- http://purl.obolibrary.org/obo/GAZ_00068137 -->

    <owl:NamedIndividual rdf:about="http://purl.obolibrary.org/obo/GAZ_00068137">
        <rdf:type rdf:resource="http://purl.obolibrary.org/obo/ENVO_00000856"/>
        <obo:RO_0001025 rdf:resource="http://purl.obolibrary.org/obo/GAZ_00000483"/>
        <obo:IAO_0000115>A municipality in the Guatemalan Department of Huehuetenango.</obo:IAO_0000115>
        <oboInOwl:hasOBONamespace>GAZ</oboInOwl:hasOBONamespace>
        <oboInOwl:id>GAZ:00068137</oboInOwl:id>
        <rdfs:label>Municipality of San Gaspar Ixchil</rdfs:label>
    </owl:NamedIndividual>
    


    <!-- http://purl.obolibrary.org/obo/GAZ_00068138 -->

    <owl:NamedIndividual rdf:about="http://purl.obolibrary.org/obo/GAZ_00068138">
        <rdf:type rdf:resource="http://purl.obolibrary.org/obo/ENVO_00000856"/>
        <obo:RO_0001025 rdf:resource="http://purl.obolibrary.org/obo/GAZ_00000483"/>
        <obo:IAO_0000115>A municipality in the Guatemalan Department of Huehuetenango.</obo:IAO_0000115>
        <oboInOwl:hasOBONamespace>GAZ</oboInOwl:hasOBONamespace>
        <oboInOwl:id>GAZ:00068138</oboInOwl:id>
        <rdfs:label>Municipality of San Juan Atitan</rdfs:label>
    </owl:NamedIndividual>
    


    <!-- http://purl.obolibrary.org/obo/GAZ_00068139 -->

    <owl:NamedIndividual rdf:about="http://purl.obolibrary.org/obo/GAZ_00068139">
        <rdf:type rdf:resource="http://purl.obolibrary.org/obo/ENVO_00000856"/>
        <obo:RO_0001025 rdf:resource="http://purl.obolibrary.org/obo/GAZ_00000483"/>
        <obo:IAO_0000115>A municipality in the Guatemalan Department of Huehuetenango.</obo:IAO_0000115>
        <oboInOwl:hasOBONamespace>GAZ</oboInOwl:hasOBONamespace>
        <oboInOwl:id>GAZ:00068139</oboInOwl:id>
        <rdfs:label>Municipality of San Mateo Ixtatan</rdfs:label>
    </owl:NamedIndividual>
    


    <!-- http://purl.obolibrary.org/obo/GAZ_00068140 -->

    <owl:NamedIndividual rdf:about="http://purl.obolibrary.org/obo/GAZ_00068140">
        <rdf:type rdf:resource="http://purl.obolibrary.org/obo/ENVO_00000856"/>
        <obo:RO_0001025 rdf:resource="http://purl.obolibrary.org/obo/GAZ_00000483"/>
        <obo:IAO_0000115>A municipality in the Guatemalan Department of Huehuetenango.</obo:IAO_0000115>
        <oboInOwl:hasOBONamespace>GAZ</oboInOwl:hasOBONamespace>
        <oboInOwl:id>GAZ:00068140</oboInOwl:id>
        <rdfs:label>Municipality of San Miguel Acatan</rdfs:label>
    </owl:NamedIndividual>
    


    <!-- http://purl.obolibrary.org/obo/GAZ_00068141 -->

    <owl:NamedIndividual rdf:about="http://purl.obolibrary.org/obo/GAZ_00068141">
        <rdf:type rdf:resource="http://purl.obolibrary.org/obo/ENVO_00000856"/>
        <obo:RO_0001025 rdf:resource="http://purl.obolibrary.org/obo/GAZ_00000483"/>
        <obo:IAO_0000115>A municipality in the Guatemalan Department of Huehuetenango.</obo:IAO_0000115>
        <oboInOwl:hasOBONamespace>GAZ</oboInOwl:hasOBONamespace>
        <oboInOwl:id>GAZ:00068141</oboInOwl:id>
        <rdfs:label>Municipality of San Sebastian Coatan</rdfs:label>
    </owl:NamedIndividual>
    


    <!-- http://purl.obolibrary.org/obo/GAZ_00068142 -->

    <owl:NamedIndividual rdf:about="http://purl.obolibrary.org/obo/GAZ_00068142">
        <rdf:type rdf:resource="http://purl.obolibrary.org/obo/ENVO_00000856"/>
        <obo:RO_0001025 rdf:resource="http://purl.obolibrary.org/obo/GAZ_00000483"/>
        <obo:IAO_0000115>A municipality in the Guatemalan Department of Huehuetenango.</obo:IAO_0000115>
        <oboInOwl:hasOBONamespace>GAZ</oboInOwl:hasOBONamespace>
        <oboInOwl:id>GAZ:00068142</oboInOwl:id>
        <rdfs:label>Municipality of Santa Ana Huista</rdfs:label>
    </owl:NamedIndividual>
    


    <!-- http://purl.obolibrary.org/obo/GAZ_00068143 -->

    <owl:NamedIndividual rdf:about="http://purl.obolibrary.org/obo/GAZ_00068143">
        <rdf:type rdf:resource="http://purl.obolibrary.org/obo/ENVO_00000856"/>
        <obo:RO_0001025 rdf:resource="http://purl.obolibrary.org/obo/GAZ_00000483"/>
        <obo:IAO_0000115>A municipality in the Guatemalan Department of Huehuetenango.</obo:IAO_0000115>
        <oboInOwl:hasOBONamespace>GAZ</oboInOwl:hasOBONamespace>
        <oboInOwl:id>GAZ:00068143</oboInOwl:id>
        <rdfs:label>Municipality of San Rafael Petzal</rdfs:label>
    </owl:NamedIndividual>
    


    <!-- http://purl.obolibrary.org/obo/GAZ_00068144 -->

    <owl:NamedIndividual rdf:about="http://purl.obolibrary.org/obo/GAZ_00068144">
        <rdf:type rdf:resource="http://purl.obolibrary.org/obo/ENVO_00000856"/>
        <obo:RO_0001025 rdf:resource="http://purl.obolibrary.org/obo/GAZ_00000483"/>
        <obo:IAO_0000115>A municipality in the Guatemalan Department of Huehuetenango.</obo:IAO_0000115>
        <oboInOwl:hasOBONamespace>GAZ</oboInOwl:hasOBONamespace>
        <oboInOwl:id>GAZ:00068144</oboInOwl:id>
        <rdfs:label>Municipality of San Pedro Necta</rdfs:label>
    </owl:NamedIndividual>
    


    <!-- http://purl.obolibrary.org/obo/GAZ_00068145 -->

    <owl:NamedIndividual rdf:about="http://purl.obolibrary.org/obo/GAZ_00068145">
        <rdf:type rdf:resource="http://purl.obolibrary.org/obo/ENVO_00000856"/>
        <obo:RO_0001025 rdf:resource="http://purl.obolibrary.org/obo/GAZ_00000483"/>
        <obo:IAO_0000115>A municipality in the Guatemalan Department of Huehuetenango.</obo:IAO_0000115>
        <oboInOwl:hasOBONamespace>GAZ</oboInOwl:hasOBONamespace>
        <oboInOwl:id>GAZ:00068145</oboInOwl:id>
        <rdfs:label>Municipality of San Rafael La Independencia</rdfs:label>
    </owl:NamedIndividual>
    


    <!-- http://purl.obolibrary.org/obo/GAZ_00068146 -->

    <owl:NamedIndividual rdf:about="http://purl.obolibrary.org/obo/GAZ_00068146">
        <rdf:type rdf:resource="http://purl.obolibrary.org/obo/ENVO_00000856"/>
        <obo:RO_0001025 rdf:resource="http://purl.obolibrary.org/obo/GAZ_00000483"/>
        <obo:IAO_0000115>A municipality in the Guatemalan Department of Huehuetenango.</obo:IAO_0000115>
        <oboInOwl:hasOBONamespace>GAZ</oboInOwl:hasOBONamespace>
        <oboInOwl:id>GAZ:00068146</oboInOwl:id>
        <rdfs:label>Municipality of San Pedro Soloma</rdfs:label>
    </owl:NamedIndividual>
    


    <!-- http://purl.obolibrary.org/obo/GAZ_00068147 -->

    <owl:NamedIndividual rdf:about="http://purl.obolibrary.org/obo/GAZ_00068147">
        <rdf:type rdf:resource="http://purl.obolibrary.org/obo/ENVO_00000856"/>
        <obo:RO_0001025 rdf:resource="http://purl.obolibrary.org/obo/GAZ_00000483"/>
        <obo:IAO_0000115>A municipality in the Guatemalan Department of Huehuetenango.</obo:IAO_0000115>
        <oboInOwl:hasOBONamespace>GAZ</oboInOwl:hasOBONamespace>
        <oboInOwl:id>GAZ:00068147</oboInOwl:id>
        <rdfs:label>Municipality of Tectitan</rdfs:label>
    </owl:NamedIndividual>
    


    <!-- http://purl.obolibrary.org/obo/GAZ_00068148 -->

    <owl:NamedIndividual rdf:about="http://purl.obolibrary.org/obo/GAZ_00068148">
        <rdf:type rdf:resource="http://purl.obolibrary.org/obo/ENVO_00000856"/>
        <obo:RO_0001025 rdf:resource="http://purl.obolibrary.org/obo/GAZ_00000483"/>
        <obo:IAO_0000115>A municipality in the Guatemalan Department of Huehuetenango.</obo:IAO_0000115>
        <oboInOwl:hasOBONamespace>GAZ</oboInOwl:hasOBONamespace>
        <oboInOwl:id>GAZ:00068148</oboInOwl:id>
        <rdfs:label>Municipality of Santa Eulalia</rdfs:label>
    </owl:NamedIndividual>
    


    <!-- http://purl.obolibrary.org/obo/GAZ_00068149 -->

    <owl:NamedIndividual rdf:about="http://purl.obolibrary.org/obo/GAZ_00068149">
        <rdf:type rdf:resource="http://purl.obolibrary.org/obo/ENVO_00000856"/>
        <obo:RO_0001025 rdf:resource="http://purl.obolibrary.org/obo/GAZ_00000483"/>
        <obo:IAO_0000115>A municipality in the Guatemalan Department of Huehuetenango.</obo:IAO_0000115>
        <oboInOwl:hasOBONamespace>GAZ</oboInOwl:hasOBONamespace>
        <oboInOwl:id>GAZ:00068149</oboInOwl:id>
        <rdfs:label>Municipality of Santiago Chimaltenango</rdfs:label>
    </owl:NamedIndividual>
    


    <!-- http://purl.obolibrary.org/obo/GAZ_00068150 -->

    <owl:NamedIndividual rdf:about="http://purl.obolibrary.org/obo/GAZ_00068150">
        <rdf:type rdf:resource="http://purl.obolibrary.org/obo/ENVO_00000856"/>
        <obo:RO_0001025 rdf:resource="http://purl.obolibrary.org/obo/GAZ_00000494"/>
        <obo:IAO_0000115>A municipality in the Izabal Department of Guatemala.</obo:IAO_0000115>
        <oboInOwl:hasOBONamespace>GAZ</oboInOwl:hasOBONamespace>
        <oboInOwl:id>GAZ:00068150</oboInOwl:id>
        <rdfs:label>Municipality of Livingston</rdfs:label>
    </owl:NamedIndividual>
    


    <!-- http://purl.obolibrary.org/obo/GAZ_00068151 -->

    <owl:NamedIndividual rdf:about="http://purl.obolibrary.org/obo/GAZ_00068151">
        <rdf:type rdf:resource="http://purl.obolibrary.org/obo/ENVO_00000856"/>
        <obo:RO_0001025 rdf:resource="http://purl.obolibrary.org/obo/GAZ_00000483"/>
        <obo:IAO_0000115>A municipality in the Guatemalan Department of Huehuetenango.</obo:IAO_0000115>
        <oboInOwl:hasOBONamespace>GAZ</oboInOwl:hasOBONamespace>
        <oboInOwl:id>GAZ:00068151</oboInOwl:id>
        <rdfs:label>Municipality of Santa Barbara</rdfs:label>
    </owl:NamedIndividual>
    


    <!-- http://purl.obolibrary.org/obo/GAZ_00068152 -->

    <owl:NamedIndividual rdf:about="http://purl.obolibrary.org/obo/GAZ_00068152">
        <rdf:type rdf:resource="http://purl.obolibrary.org/obo/ENVO_00000856"/>
        <obo:RO_0001025 rdf:resource="http://purl.obolibrary.org/obo/GAZ_00000494"/>
        <obo:IAO_0000115>A municipality in the Izabal Department of Guatemala.</obo:IAO_0000115>
        <oboInOwl:hasOBONamespace>GAZ</oboInOwl:hasOBONamespace>
        <oboInOwl:id>GAZ:00068152</oboInOwl:id>
        <rdfs:label>Municipality of El Estor</rdfs:label>
    </owl:NamedIndividual>
    


    <!-- http://purl.obolibrary.org/obo/GAZ_00068153 -->

    <owl:NamedIndividual rdf:about="http://purl.obolibrary.org/obo/GAZ_00068153">
        <rdf:type rdf:resource="http://purl.obolibrary.org/obo/ENVO_00000856"/>
        <obo:RO_0001025 rdf:resource="http://purl.obolibrary.org/obo/GAZ_00000494"/>
        <obo:IAO_0000115>A municipality in the Izabal Department of Guatemala.</obo:IAO_0000115>
        <oboInOwl:hasOBONamespace>GAZ</oboInOwl:hasOBONamespace>
        <oboInOwl:id>GAZ:00068153</oboInOwl:id>
        <rdfs:label>Municipality of Los Amates</rdfs:label>
    </owl:NamedIndividual>
    


    <!-- http://purl.obolibrary.org/obo/GAZ_00068154 -->

    <owl:NamedIndividual rdf:about="http://purl.obolibrary.org/obo/GAZ_00068154">
        <rdf:type rdf:resource="http://purl.obolibrary.org/obo/ENVO_00000856"/>
        <obo:RO_0001025 rdf:resource="http://purl.obolibrary.org/obo/GAZ_00000494"/>
        <obo:IAO_0000115>A municipality in the Izabal Department of Guatemala.</obo:IAO_0000115>
        <oboInOwl:hasOBONamespace>GAZ</oboInOwl:hasOBONamespace>
        <oboInOwl:id>GAZ:00068154</oboInOwl:id>
        <rdfs:label>Municipality of Puerto Barrios</rdfs:label>
    </owl:NamedIndividual>
    


    <!-- http://purl.obolibrary.org/obo/GAZ_00068155 -->

    <owl:NamedIndividual rdf:about="http://purl.obolibrary.org/obo/GAZ_00068155">
        <rdf:type rdf:resource="http://purl.obolibrary.org/obo/ENVO_00000856"/>
        <obo:RO_0001025 rdf:resource="http://purl.obolibrary.org/obo/GAZ_00000496"/>
        <obo:IAO_0000115>A municipality in the Jalapa Department of Guatemala.</obo:IAO_0000115>
        <oboInOwl:hasOBONamespace>GAZ</oboInOwl:hasOBONamespace>
        <oboInOwl:id>GAZ:00068155</oboInOwl:id>
        <rdfs:label>Municipality of Jalapa</rdfs:label>
    </owl:NamedIndividual>
    


    <!-- http://purl.obolibrary.org/obo/GAZ_00068156 -->

    <owl:NamedIndividual rdf:about="http://purl.obolibrary.org/obo/GAZ_00068156">
        <rdf:type rdf:resource="http://purl.obolibrary.org/obo/ENVO_00000856"/>
        <obo:RO_0001025 rdf:resource="http://purl.obolibrary.org/obo/GAZ_00000496"/>
        <obo:IAO_0000115>A municipality in the Jalapa Department of Guatemala.</obo:IAO_0000115>
        <oboInOwl:hasOBONamespace>GAZ</oboInOwl:hasOBONamespace>
        <oboInOwl:id>GAZ:00068156</oboInOwl:id>
        <rdfs:label>Municipality of San Pedro Pinula</rdfs:label>
    </owl:NamedIndividual>
    


    <!-- http://purl.obolibrary.org/obo/GAZ_00068157 -->

    <owl:NamedIndividual rdf:about="http://purl.obolibrary.org/obo/GAZ_00068157">
        <rdf:type rdf:resource="http://purl.obolibrary.org/obo/ENVO_00000856"/>
        <obo:RO_0001025 rdf:resource="http://purl.obolibrary.org/obo/GAZ_00000496"/>
        <obo:IAO_0000115>A municipality in the Jalapa Department of Guatemala.</obo:IAO_0000115>
        <oboInOwl:hasOBONamespace>GAZ</oboInOwl:hasOBONamespace>
        <oboInOwl:id>GAZ:00068157</oboInOwl:id>
        <rdfs:label>Municipality of San Carlos Alzatate</rdfs:label>
    </owl:NamedIndividual>
    


    <!-- http://purl.obolibrary.org/obo/GAZ_00068158 -->

    <owl:NamedIndividual rdf:about="http://purl.obolibrary.org/obo/GAZ_00068158">
        <rdf:type rdf:resource="http://purl.obolibrary.org/obo/ENVO_00000856"/>
        <obo:RO_0001025 rdf:resource="http://purl.obolibrary.org/obo/GAZ_00000496"/>
        <obo:IAO_0000115>A municipality in the Jalapa Department of Guatemala.</obo:IAO_0000115>
        <oboInOwl:hasOBONamespace>GAZ</oboInOwl:hasOBONamespace>
        <oboInOwl:id>GAZ:00068158</oboInOwl:id>
        <rdfs:label>Municipality of San Manuel Chaparron</rdfs:label>
    </owl:NamedIndividual>
    


    <!-- http://purl.obolibrary.org/obo/GAZ_00068159 -->

    <owl:NamedIndividual rdf:about="http://purl.obolibrary.org/obo/GAZ_00068159">
        <rdf:type rdf:resource="http://purl.obolibrary.org/obo/ENVO_00000856"/>
        <obo:RO_0001025 rdf:resource="http://purl.obolibrary.org/obo/GAZ_00000496"/>
        <obo:IAO_0000115>A municipality in the Jalapa Department of Guatemala.</obo:IAO_0000115>
        <oboInOwl:hasOBONamespace>GAZ</oboInOwl:hasOBONamespace>
        <oboInOwl:id>GAZ:00068159</oboInOwl:id>
        <rdfs:label>Municipality of San Luis Jilotepeque</rdfs:label>
    </owl:NamedIndividual>
    


    <!-- http://purl.obolibrary.org/obo/GAZ_00068160 -->

    <owl:NamedIndividual rdf:about="http://purl.obolibrary.org/obo/GAZ_00068160">
        <rdf:type rdf:resource="http://purl.obolibrary.org/obo/ENVO_00000856"/>
        <obo:RO_0001025 rdf:resource="http://purl.obolibrary.org/obo/GAZ_00000499"/>
        <obo:IAO_0000115>A municipality in the Jutiapa Department of Guatemala.</obo:IAO_0000115>
        <oboInOwl:hasOBONamespace>GAZ</oboInOwl:hasOBONamespace>
        <oboInOwl:id>GAZ:00068160</oboInOwl:id>
        <rdfs:label>Municipality of Atescatempa</rdfs:label>
    </owl:NamedIndividual>
    


    <!-- http://purl.obolibrary.org/obo/GAZ_00068161 -->

    <owl:NamedIndividual rdf:about="http://purl.obolibrary.org/obo/GAZ_00068161">
        <rdf:type rdf:resource="http://purl.obolibrary.org/obo/ENVO_00000856"/>
        <obo:RO_0001025 rdf:resource="http://purl.obolibrary.org/obo/GAZ_00000499"/>
        <obo:IAO_0000115>A municipality in the Jutiapa Department of Guatemala.</obo:IAO_0000115>
        <oboInOwl:hasOBONamespace>GAZ</oboInOwl:hasOBONamespace>
        <oboInOwl:id>GAZ:00068161</oboInOwl:id>
        <rdfs:label>Municipality of San Jose Acatempa</rdfs:label>
    </owl:NamedIndividual>
    


    <!-- http://purl.obolibrary.org/obo/GAZ_00068162 -->

    <owl:NamedIndividual rdf:about="http://purl.obolibrary.org/obo/GAZ_00068162">
        <rdf:type rdf:resource="http://purl.obolibrary.org/obo/ENVO_00000856"/>
        <obo:RO_0001025 rdf:resource="http://purl.obolibrary.org/obo/GAZ_00000499"/>
        <obo:IAO_0000115>A municipality in the Jutiapa Department of Guatemala.</obo:IAO_0000115>
        <oboInOwl:hasOBONamespace>GAZ</oboInOwl:hasOBONamespace>
        <oboInOwl:id>GAZ:00068162</oboInOwl:id>
        <rdfs:label>Municipality of Moyuta</rdfs:label>
    </owl:NamedIndividual>
    


    <!-- http://purl.obolibrary.org/obo/GAZ_00068163 -->

    <owl:NamedIndividual rdf:about="http://purl.obolibrary.org/obo/GAZ_00068163">
        <rdf:type rdf:resource="http://purl.obolibrary.org/obo/ENVO_00000856"/>
        <obo:RO_0001025 rdf:resource="http://purl.obolibrary.org/obo/GAZ_00000499"/>
        <obo:IAO_0000115>A municipality in the Jutiapa Department of Guatemala.</obo:IAO_0000115>
        <oboInOwl:hasOBONamespace>GAZ</oboInOwl:hasOBONamespace>
        <oboInOwl:id>GAZ:00068163</oboInOwl:id>
        <rdfs:label>Municipality of Conguaco</rdfs:label>
    </owl:NamedIndividual>
    


    <!-- http://purl.obolibrary.org/obo/GAZ_00068164 -->

    <owl:NamedIndividual rdf:about="http://purl.obolibrary.org/obo/GAZ_00068164">
        <rdf:type rdf:resource="http://purl.obolibrary.org/obo/ENVO_00000856"/>
        <obo:RO_0001025 rdf:resource="http://purl.obolibrary.org/obo/GAZ_00000499"/>
        <obo:IAO_0000115>A municipality in the Jutiapa Department of Guatemala.</obo:IAO_0000115>
        <oboInOwl:hasOBONamespace>GAZ</oboInOwl:hasOBONamespace>
        <oboInOwl:id>GAZ:00068164</oboInOwl:id>
        <rdfs:label>Municipality of Jerez</rdfs:label>
    </owl:NamedIndividual>
    


    <!-- http://purl.obolibrary.org/obo/GAZ_00068165 -->

    <owl:NamedIndividual rdf:about="http://purl.obolibrary.org/obo/GAZ_00068165">
        <rdf:type rdf:resource="http://purl.obolibrary.org/obo/ENVO_00000856"/>
        <obo:RO_0001025 rdf:resource="http://purl.obolibrary.org/obo/GAZ_00000499"/>
        <obo:IAO_0000115>A municipality in the Jutiapa Department of Guatemala.</obo:IAO_0000115>
        <oboInOwl:hasOBONamespace>GAZ</oboInOwl:hasOBONamespace>
        <oboInOwl:id>GAZ:00068165</oboInOwl:id>
        <rdfs:label>Municipality of Jalpatagua</rdfs:label>
    </owl:NamedIndividual>
    


    <!-- http://purl.obolibrary.org/obo/GAZ_00068166 -->

    <owl:NamedIndividual rdf:about="http://purl.obolibrary.org/obo/GAZ_00068166">
        <rdf:type rdf:resource="http://purl.obolibrary.org/obo/ENVO_00000856"/>
        <obo:RO_0001025 rdf:resource="http://purl.obolibrary.org/obo/GAZ_00000499"/>
        <obo:IAO_0000115>A municipality in the Jutiapa Department of Guatemala.</obo:IAO_0000115>
        <oboInOwl:hasOBONamespace>GAZ</oboInOwl:hasOBONamespace>
        <oboInOwl:id>GAZ:00068166</oboInOwl:id>
        <rdfs:label>Municipality of Comapa</rdfs:label>
    </owl:NamedIndividual>
    


    <!-- http://purl.obolibrary.org/obo/GAZ_00068167 -->

    <owl:NamedIndividual rdf:about="http://purl.obolibrary.org/obo/GAZ_00068167">
        <rdf:type rdf:resource="http://purl.obolibrary.org/obo/ENVO_00000856"/>
        <obo:RO_0001025 rdf:resource="http://purl.obolibrary.org/obo/GAZ_00000499"/>
        <obo:IAO_0000115>A municipality in the Jutiapa Department of Guatemala.</obo:IAO_0000115>
        <oboInOwl:hasOBONamespace>GAZ</oboInOwl:hasOBONamespace>
        <oboInOwl:id>GAZ:00068167</oboInOwl:id>
        <rdfs:label>Municipality of Zapotitlan</rdfs:label>
    </owl:NamedIndividual>
    


    <!-- http://purl.obolibrary.org/obo/GAZ_00068168 -->

    <owl:NamedIndividual rdf:about="http://purl.obolibrary.org/obo/GAZ_00068168">
        <rdf:type rdf:resource="http://purl.obolibrary.org/obo/ENVO_00000856"/>
        <obo:RO_0001025 rdf:resource="http://purl.obolibrary.org/obo/GAZ_00000499"/>
        <obo:IAO_0000115>A municipality in the Jutiapa Department of Guatemala.</obo:IAO_0000115>
        <oboInOwl:hasOBONamespace>GAZ</oboInOwl:hasOBONamespace>
        <oboInOwl:id>GAZ:00068168</oboInOwl:id>
        <rdfs:label>Municipality of Yupiltepeque</rdfs:label>
    </owl:NamedIndividual>
    


    <!-- http://purl.obolibrary.org/obo/GAZ_00068169 -->

    <owl:NamedIndividual rdf:about="http://purl.obolibrary.org/obo/GAZ_00068169">
        <rdf:type rdf:resource="http://purl.obolibrary.org/obo/ENVO_00000856"/>
        <obo:RO_0001025 rdf:resource="http://purl.obolibrary.org/obo/GAZ_00000499"/>
        <obo:IAO_0000115>A municipality in the Jutiapa Department of Guatemala.</obo:IAO_0000115>
        <oboInOwl:hasOBONamespace>GAZ</oboInOwl:hasOBONamespace>
        <oboInOwl:id>GAZ:00068169</oboInOwl:id>
        <rdfs:label>Municipality of Santa Catarina Mita</rdfs:label>
    </owl:NamedIndividual>
    


    <!-- http://purl.obolibrary.org/obo/GAZ_00068170 -->

    <owl:NamedIndividual rdf:about="http://purl.obolibrary.org/obo/GAZ_00068170">
        <rdf:type rdf:resource="http://purl.obolibrary.org/obo/ENVO_00000856"/>
        <obo:RO_0001025 rdf:resource="http://purl.obolibrary.org/obo/GAZ_00000499"/>
        <obo:IAO_0000115>A municipality in the Jutiapa Department of Guatemala.</obo:IAO_0000115>
        <oboInOwl:hasOBONamespace>GAZ</oboInOwl:hasOBONamespace>
        <oboInOwl:id>GAZ:00068170</oboInOwl:id>
        <rdfs:label>Municipality of Pasaco</rdfs:label>
    </owl:NamedIndividual>
    


    <!-- http://purl.obolibrary.org/obo/GAZ_00068171 -->

    <owl:NamedIndividual rdf:about="http://purl.obolibrary.org/obo/GAZ_00068171">
        <rdf:type rdf:resource="http://purl.obolibrary.org/obo/ENVO_00000856"/>
        <obo:RO_0001025 rdf:resource="http://purl.obolibrary.org/obo/GAZ_00000499"/>
        <obo:IAO_0000115>A municipality in the Jutiapa Department of Guatemala.</obo:IAO_0000115>
        <oboInOwl:hasOBONamespace>GAZ</oboInOwl:hasOBONamespace>
        <oboInOwl:id>GAZ:00068171</oboInOwl:id>
        <rdfs:label>Municipality of El Adelanto</rdfs:label>
    </owl:NamedIndividual>
    


    <!-- http://purl.obolibrary.org/obo/GAZ_00068172 -->

    <owl:NamedIndividual rdf:about="http://purl.obolibrary.org/obo/GAZ_00068172">
        <rdf:type rdf:resource="http://purl.obolibrary.org/obo/ENVO_00000856"/>
        <obo:RO_0001025 rdf:resource="http://purl.obolibrary.org/obo/GAZ_00000508"/>
        <obo:IAO_0000115>A municipality in the El Peten Department of Guatemala.</obo:IAO_0000115>
        <oboInOwl:hasOBONamespace>GAZ</oboInOwl:hasOBONamespace>
        <oboInOwl:id>GAZ:00068172</oboInOwl:id>
        <rdfs:label>Municipality of Poptun</rdfs:label>
    </owl:NamedIndividual>
    


    <!-- http://purl.obolibrary.org/obo/GAZ_00068173 -->

    <owl:NamedIndividual rdf:about="http://purl.obolibrary.org/obo/GAZ_00068173">
        <rdf:type rdf:resource="http://purl.obolibrary.org/obo/ENVO_00000856"/>
        <obo:RO_0001025 rdf:resource="http://purl.obolibrary.org/obo/GAZ_00000508"/>
        <obo:IAO_0000115>A municipality in the El Peten Department of Guatemala.</obo:IAO_0000115>
        <oboInOwl:hasOBONamespace>GAZ</oboInOwl:hasOBONamespace>
        <oboInOwl:id>GAZ:00068173</oboInOwl:id>
        <rdfs:label>Municipality of Santa Ana</rdfs:label>
    </owl:NamedIndividual>
    


    <!-- http://purl.obolibrary.org/obo/GAZ_00068174 -->

    <owl:NamedIndividual rdf:about="http://purl.obolibrary.org/obo/GAZ_00068174">
        <rdf:type rdf:resource="http://purl.obolibrary.org/obo/ENVO_00000856"/>
        <obo:RO_0001025 rdf:resource="http://purl.obolibrary.org/obo/GAZ_00000508"/>
        <obo:IAO_0000115>A municipality in the El Peten Department of Guatemala.</obo:IAO_0000115>
        <oboInOwl:hasOBONamespace>GAZ</oboInOwl:hasOBONamespace>
        <oboInOwl:id>GAZ:00068174</oboInOwl:id>
        <rdfs:label>Municipality of Dolores</rdfs:label>
    </owl:NamedIndividual>
    


    <!-- http://purl.obolibrary.org/obo/GAZ_00068175 -->

    <owl:NamedIndividual rdf:about="http://purl.obolibrary.org/obo/GAZ_00068175">
        <rdf:type rdf:resource="http://purl.obolibrary.org/obo/ENVO_00000856"/>
        <obo:RO_0001025 rdf:resource="http://purl.obolibrary.org/obo/GAZ_00000508"/>
        <obo:IAO_0000115>A municipality in the El Peten Department of Guatemala.</obo:IAO_0000115>
        <oboInOwl:hasOBONamespace>GAZ</oboInOwl:hasOBONamespace>
        <oboInOwl:id>GAZ:00068175</oboInOwl:id>
        <rdfs:label>Municipality of La Libertad</rdfs:label>
    </owl:NamedIndividual>
    


    <!-- http://purl.obolibrary.org/obo/GAZ_00068176 -->

    <owl:NamedIndividual rdf:about="http://purl.obolibrary.org/obo/GAZ_00068176">
        <rdf:type rdf:resource="http://purl.obolibrary.org/obo/ENVO_00000856"/>
        <obo:RO_0001025 rdf:resource="http://purl.obolibrary.org/obo/GAZ_00000508"/>
        <obo:IAO_0000115>A municipality in the El Peten Department of Guatemala.</obo:IAO_0000115>
        <oboInOwl:hasOBONamespace>GAZ</oboInOwl:hasOBONamespace>
        <oboInOwl:id>GAZ:00068176</oboInOwl:id>
        <rdfs:label>Municipality of Melchor de Mencos</rdfs:label>
    </owl:NamedIndividual>
    


    <!-- http://purl.obolibrary.org/obo/GAZ_00068177 -->

    <owl:NamedIndividual rdf:about="http://purl.obolibrary.org/obo/GAZ_00068177">
        <rdf:type rdf:resource="http://purl.obolibrary.org/obo/ENVO_00000856"/>
        <obo:RO_0001025 rdf:resource="http://purl.obolibrary.org/obo/GAZ_00000508"/>
        <obo:IAO_0000115>A municipality in the El Peten Department of Guatemala.</obo:IAO_0000115>
        <oboInOwl:hasOBONamespace>GAZ</oboInOwl:hasOBONamespace>
        <oboInOwl:id>GAZ:00068177</oboInOwl:id>
        <rdfs:label>Municipality of San Francisco</rdfs:label>
    </owl:NamedIndividual>
    


    <!-- http://purl.obolibrary.org/obo/GAZ_00068178 -->

    <owl:NamedIndividual rdf:about="http://purl.obolibrary.org/obo/GAZ_00068178">
        <rdf:type rdf:resource="http://purl.obolibrary.org/obo/ENVO_00000856"/>
        <obo:RO_0001025 rdf:resource="http://purl.obolibrary.org/obo/GAZ_00000510"/>
        <obo:IAO_0000115>A municipality in the Department of Quetzaltenango, Guatemala.</obo:IAO_0000115>
        <oboInOwl:hasOBONamespace>GAZ</oboInOwl:hasOBONamespace>
        <oboInOwl:id>GAZ:00068178</oboInOwl:id>
        <rdfs:label>Municipality of San Mateo</rdfs:label>
    </owl:NamedIndividual>
    


    <!-- http://purl.obolibrary.org/obo/GAZ_00068179 -->

    <owl:NamedIndividual rdf:about="http://purl.obolibrary.org/obo/GAZ_00068179">
        <rdf:type rdf:resource="http://purl.obolibrary.org/obo/ENVO_00000856"/>
        <obo:RO_0001025 rdf:resource="http://purl.obolibrary.org/obo/GAZ_00000508"/>
        <obo:IAO_0000115>A municipality in the El Peten Department of Guatemala.</obo:IAO_0000115>
        <oboInOwl:hasOBONamespace>GAZ</oboInOwl:hasOBONamespace>
        <oboInOwl:id>GAZ:00068179</oboInOwl:id>
        <rdfs:label>Municipality of San Jose</rdfs:label>
    </owl:NamedIndividual>
    


    <!-- http://purl.obolibrary.org/obo/GAZ_00068180 -->

    <owl:NamedIndividual rdf:about="http://purl.obolibrary.org/obo/GAZ_00068180">
        <rdf:type rdf:resource="http://purl.obolibrary.org/obo/ENVO_00000856"/>
        <obo:RO_0001025 rdf:resource="http://purl.obolibrary.org/obo/GAZ_00000508"/>
        <obo:IAO_0000115>A municipality in the El Peten Department of Guatemala.</obo:IAO_0000115>
        <oboInOwl:hasOBONamespace>GAZ</oboInOwl:hasOBONamespace>
        <oboInOwl:id>GAZ:00068180</oboInOwl:id>
        <rdfs:label>Municipality of San Andres</rdfs:label>
    </owl:NamedIndividual>
    


    <!-- http://purl.obolibrary.org/obo/GAZ_00068181 -->

    <owl:NamedIndividual rdf:about="http://purl.obolibrary.org/obo/GAZ_00068181">
        <rdf:type rdf:resource="http://purl.obolibrary.org/obo/ENVO_00000856"/>
        <obo:RO_0001025 rdf:resource="http://purl.obolibrary.org/obo/GAZ_00000508"/>
        <obo:IAO_0000115>A municipality in the El Peten Department of Guatemala.</obo:IAO_0000115>
        <oboInOwl:hasOBONamespace>GAZ</oboInOwl:hasOBONamespace>
        <oboInOwl:id>GAZ:00068181</oboInOwl:id>
        <rdfs:label>Municipality of San Luis</rdfs:label>
    </owl:NamedIndividual>
    


    <!-- http://purl.obolibrary.org/obo/GAZ_00068182 -->

    <owl:NamedIndividual rdf:about="http://purl.obolibrary.org/obo/GAZ_00068182">
        <rdf:type rdf:resource="http://purl.obolibrary.org/obo/ENVO_00000856"/>
        <obo:RO_0001025 rdf:resource="http://purl.obolibrary.org/obo/GAZ_00000508"/>
        <obo:IAO_0000115>A municipality in the El Peten Department of Guatemala.</obo:IAO_0000115>
        <oboInOwl:hasOBONamespace>GAZ</oboInOwl:hasOBONamespace>
        <oboInOwl:id>GAZ:00068182</oboInOwl:id>
        <rdfs:label>Municipality of Flores</rdfs:label>
    </owl:NamedIndividual>
    


    <!-- http://purl.obolibrary.org/obo/GAZ_00068183 -->

    <owl:NamedIndividual rdf:about="http://purl.obolibrary.org/obo/GAZ_00068183">
        <rdf:type rdf:resource="http://purl.obolibrary.org/obo/ENVO_00000856"/>
        <obo:RO_0001025 rdf:resource="http://purl.obolibrary.org/obo/GAZ_00000508"/>
        <obo:IAO_0000115>A municipality in the El Peten Department of Guatemala.</obo:IAO_0000115>
        <oboInOwl:hasOBONamespace>GAZ</oboInOwl:hasOBONamespace>
        <oboInOwl:id>GAZ:00068183</oboInOwl:id>
        <rdfs:label>Municipality of San Benito</rdfs:label>
    </owl:NamedIndividual>
    


    <!-- http://purl.obolibrary.org/obo/GAZ_00068184 -->

    <owl:NamedIndividual rdf:about="http://purl.obolibrary.org/obo/GAZ_00068184">
        <rdf:type rdf:resource="http://purl.obolibrary.org/obo/ENVO_00000856"/>
        <obo:RO_0001025 rdf:resource="http://purl.obolibrary.org/obo/GAZ_00000510"/>
        <obo:IAO_0000115>A municipality in the Department of Quetzaltenango, Guatemala.</obo:IAO_0000115>
        <oboInOwl:hasOBONamespace>GAZ</oboInOwl:hasOBONamespace>
        <oboInOwl:id>GAZ:00068184</oboInOwl:id>
        <rdfs:label>Municipality of San Martin Sacatepequez</rdfs:label>
    </owl:NamedIndividual>
    


    <!-- http://purl.obolibrary.org/obo/GAZ_00068185 -->

    <owl:NamedIndividual rdf:about="http://purl.obolibrary.org/obo/GAZ_00068185">
        <rdf:type rdf:resource="http://purl.obolibrary.org/obo/ENVO_00000856"/>
        <obo:RO_0001025 rdf:resource="http://purl.obolibrary.org/obo/GAZ_00000510"/>
        <obo:IAO_0000115>A municipality in the Quetzaltenango Department of Guatemala.</obo:IAO_0000115>
        <oboInOwl:hasOBONamespace>GAZ</oboInOwl:hasOBONamespace>
        <oboInOwl:id>GAZ:00068185</oboInOwl:id>
        <rdfs:label>Municipality of Concepcion Chiquirichapa</rdfs:label>
    </owl:NamedIndividual>
    


    <!-- http://purl.obolibrary.org/obo/GAZ_00068186 -->

    <owl:NamedIndividual rdf:about="http://purl.obolibrary.org/obo/GAZ_00068186">
        <rdf:type rdf:resource="http://purl.obolibrary.org/obo/ENVO_00000856"/>
        <obo:RO_0001025 rdf:resource="http://purl.obolibrary.org/obo/GAZ_00000510"/>
        <obo:IAO_0000115>A municipality in the Quetzaltenango Department of Guatemala.</obo:IAO_0000115>
        <oboInOwl:hasOBONamespace>GAZ</oboInOwl:hasOBONamespace>
        <oboInOwl:id>GAZ:00068186</oboInOwl:id>
        <rdfs:label>Municipality of Flores Costa Cuca</rdfs:label>
    </owl:NamedIndividual>
    


    <!-- http://purl.obolibrary.org/obo/GAZ_00068187 -->

    <owl:NamedIndividual rdf:about="http://purl.obolibrary.org/obo/GAZ_00068187">
        <rdf:type rdf:resource="http://purl.obolibrary.org/obo/ENVO_00000856"/>
        <obo:RO_0001025 rdf:resource="http://purl.obolibrary.org/obo/GAZ_00000510"/>
        <obo:IAO_0000115>A municipality in the Quetzaltenango Department of Guatemala.</obo:IAO_0000115>
        <oboInOwl:hasOBONamespace>GAZ</oboInOwl:hasOBONamespace>
        <oboInOwl:id>GAZ:00068187</oboInOwl:id>
        <rdfs:label>Municipality of Cantel</rdfs:label>
    </owl:NamedIndividual>
    


    <!-- http://purl.obolibrary.org/obo/GAZ_00068188 -->

    <owl:NamedIndividual rdf:about="http://purl.obolibrary.org/obo/GAZ_00068188">
        <rdf:type rdf:resource="http://purl.obolibrary.org/obo/ENVO_00000856"/>
        <obo:RO_0001025 rdf:resource="http://purl.obolibrary.org/obo/GAZ_00000510"/>
        <obo:IAO_0000115>A municipality in the Quetzaltenango Department of Guatemala.</obo:IAO_0000115>
        <oboInOwl:hasOBONamespace>GAZ</oboInOwl:hasOBONamespace>
        <oboInOwl:id>GAZ:00068188</oboInOwl:id>
        <rdfs:label>Municipality of Huitan</rdfs:label>
    </owl:NamedIndividual>
    


    <!-- http://purl.obolibrary.org/obo/GAZ_00068189 -->

    <owl:NamedIndividual rdf:about="http://purl.obolibrary.org/obo/GAZ_00068189">
        <rdf:type rdf:resource="http://purl.obolibrary.org/obo/ENVO_00000856"/>
        <obo:RO_0001025 rdf:resource="http://purl.obolibrary.org/obo/GAZ_00000510"/>
        <obo:IAO_0000115>A municipality in the Department of Quetzaltenango, Guatemala.</obo:IAO_0000115>
        <oboInOwl:hasOBONamespace>GAZ</oboInOwl:hasOBONamespace>
        <oboInOwl:id>GAZ:00068189</oboInOwl:id>
        <rdfs:label>Municipality of Zunil</rdfs:label>
    </owl:NamedIndividual>
    


    <!-- http://purl.obolibrary.org/obo/GAZ_00068190 -->

    <owl:NamedIndividual rdf:about="http://purl.obolibrary.org/obo/GAZ_00068190">
        <rdf:type rdf:resource="http://purl.obolibrary.org/obo/ENVO_00000856"/>
        <obo:RO_0001025 rdf:resource="http://purl.obolibrary.org/obo/GAZ_00000510"/>
        <obo:IAO_0000115>A municipality in the Quetzaltenango Department of Guatemala.</obo:IAO_0000115>
        <oboInOwl:hasOBONamespace>GAZ</oboInOwl:hasOBONamespace>
        <oboInOwl:id>GAZ:00068190</oboInOwl:id>
        <rdfs:label>Municipality of Colomba</rdfs:label>
    </owl:NamedIndividual>
    


    <!-- http://purl.obolibrary.org/obo/GAZ_00068191 -->

    <owl:NamedIndividual rdf:about="http://purl.obolibrary.org/obo/GAZ_00068191">
        <rdf:type rdf:resource="http://purl.obolibrary.org/obo/ENVO_00000856"/>
        <obo:RO_0001025 rdf:resource="http://purl.obolibrary.org/obo/GAZ_00000510"/>
        <obo:IAO_0000115>A municipality in the Quetzaltenango Department of Guatemala.</obo:IAO_0000115>
        <oboInOwl:hasOBONamespace>GAZ</oboInOwl:hasOBONamespace>
        <oboInOwl:id>GAZ:00068191</oboInOwl:id>
        <rdfs:label>Municipality of La Esperanza</rdfs:label>
    </owl:NamedIndividual>
    


    <!-- http://purl.obolibrary.org/obo/GAZ_00068192 -->

    <owl:NamedIndividual rdf:about="http://purl.obolibrary.org/obo/GAZ_00068192">
        <rdf:type rdf:resource="http://purl.obolibrary.org/obo/ENVO_00000856"/>
        <obo:RO_0001025 rdf:resource="http://purl.obolibrary.org/obo/GAZ_00000510"/>
        <obo:IAO_0000115>A municipality in the Quetzaltenango Department of Guatemala.</obo:IAO_0000115>
        <oboInOwl:hasOBONamespace>GAZ</oboInOwl:hasOBONamespace>
        <oboInOwl:id>GAZ:00068192</oboInOwl:id>
        <rdfs:label>Municipality of El Palmar</rdfs:label>
    </owl:NamedIndividual>
    


    <!-- http://purl.obolibrary.org/obo/GAZ_00068193 -->

    <owl:NamedIndividual rdf:about="http://purl.obolibrary.org/obo/GAZ_00068193">
        <rdf:type rdf:resource="http://purl.obolibrary.org/obo/ENVO_00000856"/>
        <obo:RO_0001025 rdf:resource="http://purl.obolibrary.org/obo/GAZ_00000510"/>
        <obo:IAO_0000115>A municipality in the Quetzaltenango Department of Guatemala.</obo:IAO_0000115>
        <oboInOwl:hasOBONamespace>GAZ</oboInOwl:hasOBONamespace>
        <oboInOwl:id>GAZ:00068193</oboInOwl:id>
        <rdfs:label>Municipality of Genova</rdfs:label>
    </owl:NamedIndividual>
    


    <!-- http://purl.obolibrary.org/obo/GAZ_00068194 -->

    <owl:NamedIndividual rdf:about="http://purl.obolibrary.org/obo/GAZ_00068194">
        <rdf:type rdf:resource="http://purl.obolibrary.org/obo/ENVO_00000856"/>
        <obo:RO_0001025 rdf:resource="http://purl.obolibrary.org/obo/GAZ_00000510"/>
        <obo:IAO_0000115>A municipality in the Department of Quetzaltenango, Guatemala.</obo:IAO_0000115>
        <oboInOwl:hasOBONamespace>GAZ</oboInOwl:hasOBONamespace>
        <oboInOwl:id>GAZ:00068194</oboInOwl:id>
        <rdfs:label>Municipality of San Miguel Siguila</rdfs:label>
    </owl:NamedIndividual>
    


    <!-- http://purl.obolibrary.org/obo/GAZ_00068195 -->

    <owl:NamedIndividual rdf:about="http://purl.obolibrary.org/obo/GAZ_00068195">
        <rdf:type rdf:resource="http://purl.obolibrary.org/obo/ENVO_00000856"/>
        <obo:RO_0001025 rdf:resource="http://purl.obolibrary.org/obo/GAZ_00000510"/>
        <obo:IAO_0000115>A municipality in the Quetzaltenango Department of Guatemala.</obo:IAO_0000115>
        <oboInOwl:hasOBONamespace>GAZ</oboInOwl:hasOBONamespace>
        <oboInOwl:id>GAZ:00068195</oboInOwl:id>
        <rdfs:label>Municipality of Olintepeque</rdfs:label>
    </owl:NamedIndividual>
    


    <!-- http://purl.obolibrary.org/obo/GAZ_00068196 -->

    <owl:NamedIndividual rdf:about="http://purl.obolibrary.org/obo/GAZ_00068196">
        <obo:RO_0001025 rdf:resource="http://purl.obolibrary.org/obo/GAZ_00000510"/>
        <obo:IAO_0000115>A municipality in the Department of Quetzaltenango, Guatemala.</obo:IAO_0000115>
        <oboInOwl:hasOBONamespace>GAZ</oboInOwl:hasOBONamespace>
        <oboInOwl:id>GAZ:00068196</oboInOwl:id>
        <rdfs:label>Municipality of Sibilia</rdfs:label>
    </owl:NamedIndividual>
    


    <!-- http://purl.obolibrary.org/obo/GAZ_00068197 -->

    <owl:NamedIndividual rdf:about="http://purl.obolibrary.org/obo/GAZ_00068197">
        <rdf:type rdf:resource="http://purl.obolibrary.org/obo/ENVO_00000856"/>
        <obo:RO_0001025 rdf:resource="http://purl.obolibrary.org/obo/GAZ_00000510"/>
        <obo:IAO_0000115>A municipality in the Quetzaltenango Department of Guatemala.</obo:IAO_0000115>
        <oboInOwl:hasOBONamespace>GAZ</oboInOwl:hasOBONamespace>
        <oboInOwl:id>GAZ:00068197</oboInOwl:id>
        <rdfs:label>Municipality of Coatepeque</rdfs:label>
    </owl:NamedIndividual>
    


    <!-- http://purl.obolibrary.org/obo/GAZ_00068198 -->

    <owl:NamedIndividual rdf:about="http://purl.obolibrary.org/obo/GAZ_00068198">
        <rdf:type rdf:resource="http://purl.obolibrary.org/obo/ENVO_00000856"/>
        <obo:RO_0001025 rdf:resource="http://purl.obolibrary.org/obo/GAZ_00000510"/>
        <obo:IAO_0000115>A municipality in the Quetzaltenango Department of Guatemala.</obo:IAO_0000115>
        <oboInOwl:hasOBONamespace>GAZ</oboInOwl:hasOBONamespace>
        <oboInOwl:id>GAZ:00068198</oboInOwl:id>
        <rdfs:label>Municipality of Cabrican</rdfs:label>
    </owl:NamedIndividual>
    


    <!-- http://purl.obolibrary.org/obo/GAZ_00068199 -->

    <owl:NamedIndividual rdf:about="http://purl.obolibrary.org/obo/GAZ_00068199">
        <rdf:type rdf:resource="http://purl.obolibrary.org/obo/ENVO_00000856"/>
        <obo:RO_0001025 rdf:resource="http://purl.obolibrary.org/obo/GAZ_00000510"/>
        <obo:IAO_0000115>A municipality in the Quetzaltenango Department of Guatemala.</obo:IAO_0000115>
        <oboInOwl:hasOBONamespace>GAZ</oboInOwl:hasOBONamespace>
        <oboInOwl:id>GAZ:00068199</oboInOwl:id>
        <rdfs:label>Municipality of San Juan Ostuncalco</rdfs:label>
    </owl:NamedIndividual>
    


    <!-- http://purl.obolibrary.org/obo/GAZ_00068200 -->

    <owl:NamedIndividual rdf:about="http://purl.obolibrary.org/obo/GAZ_00068200">
        <rdf:type rdf:resource="http://purl.obolibrary.org/obo/ENVO_00000856"/>
        <obo:RO_0001025 rdf:resource="http://purl.obolibrary.org/obo/GAZ_00000510"/>
        <obo:IAO_0000115>A municipality in the Quetzaltenango Department of Guatemala.</obo:IAO_0000115>
        <oboInOwl:hasOBONamespace>GAZ</oboInOwl:hasOBONamespace>
        <oboInOwl:id>GAZ:00068200</oboInOwl:id>
        <rdfs:label>Municipality of Almolonga</rdfs:label>
    </owl:NamedIndividual>
    


    <!-- http://purl.obolibrary.org/obo/GAZ_00068201 -->

    <owl:NamedIndividual rdf:about="http://purl.obolibrary.org/obo/GAZ_00068201">
        <rdf:type rdf:resource="http://purl.obolibrary.org/obo/ENVO_00000856"/>
        <obo:RO_0001025 rdf:resource="http://purl.obolibrary.org/obo/GAZ_00000510"/>
        <obo:IAO_0000115>A municipality in the Quetzaltenango Department of Guatemala.</obo:IAO_0000115>
        <oboInOwl:hasOBONamespace>GAZ</oboInOwl:hasOBONamespace>
        <oboInOwl:id>GAZ:00068201</oboInOwl:id>
        <rdfs:label>Municipality of San Francisco La Union</rdfs:label>
    </owl:NamedIndividual>
    


    <!-- http://purl.obolibrary.org/obo/GAZ_00068202 -->

    <owl:NamedIndividual rdf:about="http://purl.obolibrary.org/obo/GAZ_00068202">
        <rdf:type rdf:resource="http://purl.obolibrary.org/obo/ENVO_00000856"/>
        <obo:RO_0001025 rdf:resource="http://purl.obolibrary.org/obo/GAZ_00000510"/>
        <obo:IAO_0000115>A municipality in the Quetzaltenango Department of Guatemala.</obo:IAO_0000115>
        <oboInOwl:hasOBONamespace>GAZ</oboInOwl:hasOBONamespace>
        <oboInOwl:id>GAZ:00068202</oboInOwl:id>
        <rdfs:label>Municipality of Cajola</rdfs:label>
    </owl:NamedIndividual>
    


    <!-- http://purl.obolibrary.org/obo/GAZ_00068203 -->

    <owl:NamedIndividual rdf:about="http://purl.obolibrary.org/obo/GAZ_00068203">
        <rdf:type rdf:resource="http://purl.obolibrary.org/obo/ENVO_00000856"/>
        <obo:RO_0001025 rdf:resource="http://purl.obolibrary.org/obo/GAZ_00000517"/>
        <obo:IAO_0000115>A municipality in the Guatemalan Department of El Quiche.</obo:IAO_0000115>
        <oboInOwl:hasOBONamespace>GAZ</oboInOwl:hasOBONamespace>
        <oboInOwl:id>GAZ:00068203</oboInOwl:id>
        <rdfs:label>Municipality of Cunen</rdfs:label>
    </owl:NamedIndividual>
    


    <!-- http://purl.obolibrary.org/obo/GAZ_00068204 -->

    <owl:NamedIndividual rdf:about="http://purl.obolibrary.org/obo/GAZ_00068204">
        <rdf:type rdf:resource="http://purl.obolibrary.org/obo/ENVO_00000856"/>
        <obo:RO_0001025 rdf:resource="http://purl.obolibrary.org/obo/GAZ_00000510"/>
        <obo:IAO_0000115>A municipality in the Quetzaltenango Department of Guatemala.</obo:IAO_0000115>
        <oboInOwl:hasOBONamespace>GAZ</oboInOwl:hasOBONamespace>
        <oboInOwl:id>GAZ:00068204</oboInOwl:id>
        <rdfs:label>Municipality of San Carlos Sija</rdfs:label>
    </owl:NamedIndividual>
    


    <!-- http://purl.obolibrary.org/obo/GAZ_00068205 -->

    <owl:NamedIndividual rdf:about="http://purl.obolibrary.org/obo/GAZ_00068205">
        <rdf:type rdf:resource="http://purl.obolibrary.org/obo/ENVO_00000856"/>
        <obo:RO_0001025 rdf:resource="http://purl.obolibrary.org/obo/GAZ_00000517"/>
        <obo:IAO_0000115>A municipality in the Guatemalan Department of El Quiche.</obo:IAO_0000115>
        <oboInOwl:hasOBONamespace>GAZ</oboInOwl:hasOBONamespace>
        <oboInOwl:id>GAZ:00068205</oboInOwl:id>
        <rdfs:label>Municipality of Chiche</rdfs:label>
    </owl:NamedIndividual>
    


    <!-- http://purl.obolibrary.org/obo/GAZ_00068206 -->

    <owl:NamedIndividual rdf:about="http://purl.obolibrary.org/obo/GAZ_00068206">
        <rdf:type rdf:resource="http://purl.obolibrary.org/obo/ENVO_00000856"/>
        <obo:RO_0001025 rdf:resource="http://purl.obolibrary.org/obo/GAZ_00000510"/>
        <obo:IAO_0000115>A municipality in the Quetzaltenango Department of Guatemala.</obo:IAO_0000115>
        <oboInOwl:hasOBONamespace>GAZ</oboInOwl:hasOBONamespace>
        <oboInOwl:id>GAZ:00068206</oboInOwl:id>
        <rdfs:label>Municipality of Quetzaltenango</rdfs:label>
    </owl:NamedIndividual>
    


    <!-- http://purl.obolibrary.org/obo/GAZ_00068207 -->

    <owl:NamedIndividual rdf:about="http://purl.obolibrary.org/obo/GAZ_00068207">
        <rdf:type rdf:resource="http://purl.obolibrary.org/obo/ENVO_00000856"/>
        <obo:RO_0001025 rdf:resource="http://purl.obolibrary.org/obo/GAZ_00000510"/>
        <obo:IAO_0000115>A municipality in the Quetzaltenango Department of Guatemala.</obo:IAO_0000115>
        <oboInOwl:hasOBONamespace>GAZ</oboInOwl:hasOBONamespace>
        <oboInOwl:id>GAZ:00068207</oboInOwl:id>
        <rdfs:label>Municipality of Salcaja</rdfs:label>
    </owl:NamedIndividual>
    


    <!-- http://purl.obolibrary.org/obo/GAZ_00068208 -->

    <owl:NamedIndividual rdf:about="http://purl.obolibrary.org/obo/GAZ_00068208">
        <rdf:type rdf:resource="http://purl.obolibrary.org/obo/ENVO_00000856"/>
        <obo:RO_0001025 rdf:resource="http://purl.obolibrary.org/obo/GAZ_00000517"/>
        <obo:IAO_0000115>A municipality in the Guatemalan Department of El Quiche.</obo:IAO_0000115>
        <oboInOwl:hasOBONamespace>GAZ</oboInOwl:hasOBONamespace>
        <oboInOwl:id>GAZ:00068208</oboInOwl:id>
        <rdfs:label>Municipality of Canilla</rdfs:label>
    </owl:NamedIndividual>
    


    <!-- http://purl.obolibrary.org/obo/GAZ_00068209 -->

    <owl:NamedIndividual rdf:about="http://purl.obolibrary.org/obo/GAZ_00068209">
        <rdf:type rdf:resource="http://purl.obolibrary.org/obo/ENVO_00000856"/>
        <obo:RO_0001025 rdf:resource="http://purl.obolibrary.org/obo/GAZ_00000517"/>
        <obo:IAO_0000115>A municipality in the Guatemalan Department of El Quiche.</obo:IAO_0000115>
        <oboInOwl:hasOBONamespace>GAZ</oboInOwl:hasOBONamespace>
        <oboInOwl:id>GAZ:00068209</oboInOwl:id>
        <rdfs:label>Municipality of Chinique</rdfs:label>
    </owl:NamedIndividual>
    


    <!-- http://purl.obolibrary.org/obo/GAZ_00068210 -->

    <owl:NamedIndividual rdf:about="http://purl.obolibrary.org/obo/GAZ_00068210">
        <rdf:type rdf:resource="http://purl.obolibrary.org/obo/ENVO_00000856"/>
        <obo:RO_0001025 rdf:resource="http://purl.obolibrary.org/obo/GAZ_00000517"/>
        <obo:IAO_0000115>A municipality in the Guatemalan Department of El Quiche.</obo:IAO_0000115>
        <oboInOwl:hasOBONamespace>GAZ</oboInOwl:hasOBONamespace>
        <oboInOwl:id>GAZ:00068210</oboInOwl:id>
        <rdfs:label>Municipality of Joyabaj</rdfs:label>
    </owl:NamedIndividual>
    


    <!-- http://purl.obolibrary.org/obo/GAZ_00068211 -->

    <owl:NamedIndividual rdf:about="http://purl.obolibrary.org/obo/GAZ_00068211">
        <rdf:type rdf:resource="http://purl.obolibrary.org/obo/ENVO_00000856"/>
        <obo:RO_0001025 rdf:resource="http://purl.obolibrary.org/obo/GAZ_00000517"/>
        <obo:IAO_0000115>A municipality in the Guatemalan Department of El Quiche.</obo:IAO_0000115>
        <oboInOwl:hasOBONamespace>GAZ</oboInOwl:hasOBONamespace>
        <oboInOwl:id>GAZ:00068211</oboInOwl:id>
        <rdfs:label>Municipality of Chicaman</rdfs:label>
    </owl:NamedIndividual>
    


    <!-- http://purl.obolibrary.org/obo/GAZ_00068212 -->

    <owl:NamedIndividual rdf:about="http://purl.obolibrary.org/obo/GAZ_00068212">
        <rdf:type rdf:resource="http://purl.obolibrary.org/obo/ENVO_00000856"/>
        <obo:RO_0001025 rdf:resource="http://purl.obolibrary.org/obo/GAZ_00000517"/>
        <obo:IAO_0000115>A municipality in the El Quiche department of Guatemala.</obo:IAO_0000115>
        <oboInOwl:hasOBONamespace>GAZ</oboInOwl:hasOBONamespace>
        <oboInOwl:id>GAZ:00068212</oboInOwl:id>
        <rdfs:label>Municipality of Santo Tomas Chichicastenango</rdfs:label>
    </owl:NamedIndividual>
    


    <!-- http://purl.obolibrary.org/obo/GAZ_00068213 -->

    <owl:NamedIndividual rdf:about="http://purl.obolibrary.org/obo/GAZ_00068213">
        <rdf:type rdf:resource="http://purl.obolibrary.org/obo/ENVO_00000856"/>
        <obo:RO_0001025 rdf:resource="http://purl.obolibrary.org/obo/GAZ_00000517"/>
        <obo:IAO_0000115>A municipality in the Guatemalan Department of El Quiche.</obo:IAO_0000115>
        <oboInOwl:hasOBONamespace>GAZ</oboInOwl:hasOBONamespace>
        <oboInOwl:id>GAZ:00068213</oboInOwl:id>
        <rdfs:label>Municipality of Ixcan</rdfs:label>
    </owl:NamedIndividual>
    


    <!-- http://purl.obolibrary.org/obo/GAZ_00068214 -->

    <owl:NamedIndividual rdf:about="http://purl.obolibrary.org/obo/GAZ_00068214">
        <rdf:type rdf:resource="http://purl.obolibrary.org/obo/ENVO_00000856"/>
        <obo:RO_0001025 rdf:resource="http://purl.obolibrary.org/obo/GAZ_00000517"/>
        <obo:IAO_0000115>A municipality in the Guatemalan Department of El Quiche.</obo:IAO_0000115>
        <oboInOwl:hasOBONamespace>GAZ</oboInOwl:hasOBONamespace>
        <oboInOwl:id>GAZ:00068214</oboInOwl:id>
        <rdfs:label>Municipality of San Andres Sajcabaja</rdfs:label>
    </owl:NamedIndividual>
    


    <!-- http://purl.obolibrary.org/obo/GAZ_00068215 -->

    <owl:NamedIndividual rdf:about="http://purl.obolibrary.org/obo/GAZ_00068215">
        <rdf:type rdf:resource="http://purl.obolibrary.org/obo/ENVO_00000856"/>
        <obo:RO_0001025 rdf:resource="http://purl.obolibrary.org/obo/GAZ_00000517"/>
        <obo:IAO_0000115>A municipality in the Guatemalan Department of El Quiche.</obo:IAO_0000115>
        <oboInOwl:hasOBONamespace>GAZ</oboInOwl:hasOBONamespace>
        <oboInOwl:id>GAZ:00068215</oboInOwl:id>
        <rdfs:label>Municipality of Sacapulas</rdfs:label>
    </owl:NamedIndividual>
    


    <!-- http://purl.obolibrary.org/obo/GAZ_00068216 -->

    <owl:NamedIndividual rdf:about="http://purl.obolibrary.org/obo/GAZ_00068216">
        <rdf:type rdf:resource="http://purl.obolibrary.org/obo/ENVO_00000856"/>
        <obo:RO_0001025 rdf:resource="http://purl.obolibrary.org/obo/GAZ_00000517"/>
        <obo:IAO_0000115>A municipality in the Guatemalan Department of El Quiche.</obo:IAO_0000115>
        <oboInOwl:hasOBONamespace>GAZ</oboInOwl:hasOBONamespace>
        <oboInOwl:id>GAZ:00068216</oboInOwl:id>
        <rdfs:label>Municipality of San Juan Cotzal</rdfs:label>
    </owl:NamedIndividual>
    


    <!-- http://purl.obolibrary.org/obo/GAZ_00068217 -->

    <owl:NamedIndividual rdf:about="http://purl.obolibrary.org/obo/GAZ_00068217">
        <rdf:type rdf:resource="http://purl.obolibrary.org/obo/ENVO_00000856"/>
        <obo:RO_0001025 rdf:resource="http://purl.obolibrary.org/obo/GAZ_00000517"/>
        <obo:IAO_0000115>A municipality in the Guatemalan Department of El Quiche.</obo:IAO_0000115>
        <oboInOwl:hasOBONamespace>GAZ</oboInOwl:hasOBONamespace>
        <oboInOwl:id>GAZ:00068217</oboInOwl:id>
        <rdfs:label>Municipality of Patzite</rdfs:label>
    </owl:NamedIndividual>
    


    <!-- http://purl.obolibrary.org/obo/GAZ_00068218 -->

    <owl:NamedIndividual rdf:about="http://purl.obolibrary.org/obo/GAZ_00068218">
        <rdf:type rdf:resource="http://purl.obolibrary.org/obo/ENVO_00000856"/>
        <obo:RO_0001025 rdf:resource="http://purl.obolibrary.org/obo/GAZ_00000517"/>
        <obo:IAO_0000115>A municipality in the Guatemalan Department of El Quiche.</obo:IAO_0000115>
        <oboInOwl:hasOBONamespace>GAZ</oboInOwl:hasOBONamespace>
        <oboInOwl:id>GAZ:00068218</oboInOwl:id>
        <rdfs:label>Municipality of San Antonio Ilotenango</rdfs:label>
    </owl:NamedIndividual>
    


    <!-- http://purl.obolibrary.org/obo/GAZ_00068219 -->

    <owl:NamedIndividual rdf:about="http://purl.obolibrary.org/obo/GAZ_00068219">
        <rdf:type rdf:resource="http://purl.obolibrary.org/obo/ENVO_00000856"/>
        <obo:RO_0001025 rdf:resource="http://purl.obolibrary.org/obo/GAZ_00000517"/>
        <obo:IAO_0000115>A municipality in the Guatemalan Department of El Quiche.</obo:IAO_0000115>
        <oboInOwl:hasOBONamespace>GAZ</oboInOwl:hasOBONamespace>
        <oboInOwl:id>GAZ:00068219</oboInOwl:id>
        <rdfs:label>Municipality of Pachalum</rdfs:label>
    </owl:NamedIndividual>
    


    <!-- http://purl.obolibrary.org/obo/GAZ_00068220 -->

    <owl:NamedIndividual rdf:about="http://purl.obolibrary.org/obo/GAZ_00068220">
        <rdf:type rdf:resource="http://purl.obolibrary.org/obo/ENVO_00000856"/>
        <obo:RO_0001025 rdf:resource="http://purl.obolibrary.org/obo/GAZ_00000517"/>
        <obo:IAO_0000115>A municipality in the Guatemalan Department of El Quiche.</obo:IAO_0000115>
        <oboInOwl:hasOBONamespace>GAZ</oboInOwl:hasOBONamespace>
        <oboInOwl:id>GAZ:00068220</oboInOwl:id>
        <rdfs:label>Municipality of San Bartolome Jocotenango</rdfs:label>
    </owl:NamedIndividual>
    


    <!-- http://purl.obolibrary.org/obo/GAZ_00068221 -->

    <owl:NamedIndividual rdf:about="http://purl.obolibrary.org/obo/GAZ_00068221">
        <rdf:type rdf:resource="http://purl.obolibrary.org/obo/ENVO_00000856"/>
        <obo:RO_0001025 rdf:resource="http://purl.obolibrary.org/obo/GAZ_00000517"/>
        <obo:IAO_0000115>A municipality in the Guatemalan Department of El Quiche.</obo:IAO_0000115>
        <oboInOwl:hasOBONamespace>GAZ</oboInOwl:hasOBONamespace>
        <oboInOwl:id>GAZ:00068221</oboInOwl:id>
        <rdfs:label>Municipality of Zacualpa</rdfs:label>
    </owl:NamedIndividual>
    


    <!-- http://purl.obolibrary.org/obo/GAZ_00068222 -->

    <owl:NamedIndividual rdf:about="http://purl.obolibrary.org/obo/GAZ_00068222">
        <rdf:type rdf:resource="http://purl.obolibrary.org/obo/ENVO_00000856"/>
        <obo:RO_0001025 rdf:resource="http://purl.obolibrary.org/obo/GAZ_00000517"/>
        <obo:IAO_0000115>A municipality in the Guatemalan Department of El Quiche.</obo:IAO_0000115>
        <oboInOwl:hasOBONamespace>GAZ</oboInOwl:hasOBONamespace>
        <oboInOwl:id>GAZ:00068222</oboInOwl:id>
        <rdfs:label>Municipality of Santa Cruz del Quiche</rdfs:label>
    </owl:NamedIndividual>
    


    <!-- http://purl.obolibrary.org/obo/GAZ_00068223 -->

    <owl:NamedIndividual rdf:about="http://purl.obolibrary.org/obo/GAZ_00068223">
        <rdf:type rdf:resource="http://purl.obolibrary.org/obo/ENVO_00000856"/>
        <obo:RO_0001025 rdf:resource="http://purl.obolibrary.org/obo/GAZ_00000525"/>
        <obo:IAO_0000115>A municipality in the Guatemalan Department of Sacatepequez.</obo:IAO_0000115>
        <oboInOwl:hasOBONamespace>GAZ</oboInOwl:hasOBONamespace>
        <oboInOwl:id>GAZ:00068223</oboInOwl:id>
        <rdfs:label>Municipality of Magdalena Milpas Altas</rdfs:label>
    </owl:NamedIndividual>
    


    <!-- http://purl.obolibrary.org/obo/GAZ_00068224 -->

    <owl:NamedIndividual rdf:about="http://purl.obolibrary.org/obo/GAZ_00068224">
        <rdf:type rdf:resource="http://purl.obolibrary.org/obo/ENVO_00000856"/>
        <obo:RO_0001025 rdf:resource="http://purl.obolibrary.org/obo/GAZ_00000525"/>
        <obo:IAO_0000115>A municipality in the Guatemalan Department of Sacatepequez.</obo:IAO_0000115>
        <oboInOwl:hasOBONamespace>GAZ</oboInOwl:hasOBONamespace>
        <oboInOwl:id>GAZ:00068224</oboInOwl:id>
        <rdfs:label>Municipality of Jocotenango</rdfs:label>
    </owl:NamedIndividual>
    


    <!-- http://purl.obolibrary.org/obo/GAZ_00068225 -->

    <owl:NamedIndividual rdf:about="http://purl.obolibrary.org/obo/GAZ_00068225">
        <rdf:type rdf:resource="http://purl.obolibrary.org/obo/ENVO_00000856"/>
        <obo:RO_0001025 rdf:resource="http://purl.obolibrary.org/obo/GAZ_00000522"/>
        <obo:IAO_0000115>A municipality in the Retalhuleu Department in southwestern Guatemala.</obo:IAO_0000115>
        <oboInOwl:hasOBONamespace>GAZ</oboInOwl:hasOBONamespace>
        <oboInOwl:id>GAZ:00068225</oboInOwl:id>
        <rdfs:label>Municipality of Santa Cruz Mulua</rdfs:label>
    </owl:NamedIndividual>
    


    <!-- http://purl.obolibrary.org/obo/GAZ_00068226 -->

    <owl:NamedIndividual rdf:about="http://purl.obolibrary.org/obo/GAZ_00068226">
        <rdf:type rdf:resource="http://purl.obolibrary.org/obo/ENVO_00000856"/>
        <obo:RO_0001025 rdf:resource="http://purl.obolibrary.org/obo/GAZ_00000522"/>
        <obo:IAO_0000115>A municipality in the Retalhuleu Department in southwestern Guatemala.</obo:IAO_0000115>
        <oboInOwl:hasOBONamespace>GAZ</oboInOwl:hasOBONamespace>
        <oboInOwl:id>GAZ:00068226</oboInOwl:id>
        <rdfs:label>Municipality of Retalhuleu</rdfs:label>
    </owl:NamedIndividual>
    


    <!-- http://purl.obolibrary.org/obo/GAZ_00068227 -->

    <owl:NamedIndividual rdf:about="http://purl.obolibrary.org/obo/GAZ_00068227">
        <rdf:type rdf:resource="http://purl.obolibrary.org/obo/ENVO_00000856"/>
        <obo:RO_0001025 rdf:resource="http://purl.obolibrary.org/obo/GAZ_00000522"/>
        <obo:IAO_0000115>A municipality in the Retalhuleu Department in southwestern Guatemala.</obo:IAO_0000115>
        <oboInOwl:hasOBONamespace>GAZ</oboInOwl:hasOBONamespace>
        <oboInOwl:id>GAZ:00068227</oboInOwl:id>
        <rdfs:label>Municipality of San Martin Zapotitlan</rdfs:label>
    </owl:NamedIndividual>
    


    <!-- http://purl.obolibrary.org/obo/GAZ_00068228 -->

    <owl:NamedIndividual rdf:about="http://purl.obolibrary.org/obo/GAZ_00068228">
        <rdf:type rdf:resource="http://purl.obolibrary.org/obo/ENVO_00000856"/>
        <obo:RO_0001025 rdf:resource="http://purl.obolibrary.org/obo/GAZ_00000522"/>
        <obo:IAO_0000115>A municipality in the Retalhuleu Department in southwestern Guatemala.</obo:IAO_0000115>
        <oboInOwl:hasOBONamespace>GAZ</oboInOwl:hasOBONamespace>
        <oboInOwl:id>GAZ:00068228</oboInOwl:id>
        <rdfs:label>Municipality of Nuevo San Carlos</rdfs:label>
    </owl:NamedIndividual>
    


    <!-- http://purl.obolibrary.org/obo/GAZ_00068229 -->

    <owl:NamedIndividual rdf:about="http://purl.obolibrary.org/obo/GAZ_00068229">
        <rdf:type rdf:resource="http://purl.obolibrary.org/obo/ENVO_00000856"/>
        <obo:RO_0001025 rdf:resource="http://purl.obolibrary.org/obo/GAZ_00000522"/>
        <obo:IAO_0000115>A municipality in the Retalhuleu Department in southwestern Guatemala.</obo:IAO_0000115>
        <oboInOwl:hasOBONamespace>GAZ</oboInOwl:hasOBONamespace>
        <oboInOwl:id>GAZ:00068229</oboInOwl:id>
        <rdfs:label>Municipality of Champerico</rdfs:label>
    </owl:NamedIndividual>
    


    <!-- http://purl.obolibrary.org/obo/GAZ_00068230 -->

    <owl:NamedIndividual rdf:about="http://purl.obolibrary.org/obo/GAZ_00068230">
        <rdf:type rdf:resource="http://purl.obolibrary.org/obo/ENVO_00000856"/>
        <obo:RO_0001025 rdf:resource="http://purl.obolibrary.org/obo/GAZ_00000522"/>
        <obo:IAO_0000115>A municipality in the Retalhuleu Department in southwestern Guatemala.</obo:IAO_0000115>
        <oboInOwl:hasOBONamespace>GAZ</oboInOwl:hasOBONamespace>
        <oboInOwl:id>GAZ:00068230</oboInOwl:id>
        <rdfs:label>Municipality of San Andres Villa Seca</rdfs:label>
    </owl:NamedIndividual>
    


    <!-- http://purl.obolibrary.org/obo/GAZ_00068231 -->

    <owl:NamedIndividual rdf:about="http://purl.obolibrary.org/obo/GAZ_00068231">
        <rdf:type rdf:resource="http://purl.obolibrary.org/obo/ENVO_00000856"/>
        <obo:RO_0001025 rdf:resource="http://purl.obolibrary.org/obo/GAZ_00000522"/>
        <obo:IAO_0000115>A municipality in the Retalhuleu Department in southwestern Guatemala.</obo:IAO_0000115>
        <oboInOwl:hasOBONamespace>GAZ</oboInOwl:hasOBONamespace>
        <oboInOwl:id>GAZ:00068231</oboInOwl:id>
        <rdfs:label>Municipality of San Felipe</rdfs:label>
    </owl:NamedIndividual>
    


    <!-- http://purl.obolibrary.org/obo/GAZ_00068232 -->

    <owl:NamedIndividual rdf:about="http://purl.obolibrary.org/obo/GAZ_00068232">
        <rdf:type rdf:resource="http://purl.obolibrary.org/obo/ENVO_00000856"/>
        <obo:RO_0001025 rdf:resource="http://purl.obolibrary.org/obo/GAZ_00000522"/>
        <obo:IAO_0000115>A municipality in the Retalhuleu Department in southwestern Guatemala.</obo:IAO_0000115>
        <oboInOwl:hasOBONamespace>GAZ</oboInOwl:hasOBONamespace>
        <oboInOwl:id>GAZ:00068232</oboInOwl:id>
        <rdfs:label>Municipality of San Sebastian</rdfs:label>
    </owl:NamedIndividual>
    


    <!-- http://purl.obolibrary.org/obo/GAZ_00068233 -->

    <owl:NamedIndividual rdf:about="http://purl.obolibrary.org/obo/GAZ_00068233">
        <rdf:type rdf:resource="http://purl.obolibrary.org/obo/ENVO_00000856"/>
        <obo:RO_0001025 rdf:resource="http://purl.obolibrary.org/obo/GAZ_00000525"/>
        <obo:IAO_0000115>A municipality in the Guatemalan Department of Sacatepequez.</obo:IAO_0000115>
        <oboInOwl:hasOBONamespace>GAZ</oboInOwl:hasOBONamespace>
        <oboInOwl:id>GAZ:00068233</oboInOwl:id>
        <rdfs:label>Municipality of Pastores</rdfs:label>
    </owl:NamedIndividual>
    


    <!-- http://purl.obolibrary.org/obo/GAZ_00068234 -->

    <owl:NamedIndividual rdf:about="http://purl.obolibrary.org/obo/GAZ_00068234">
        <rdf:type rdf:resource="http://purl.obolibrary.org/obo/ENVO_00000856"/>
        <obo:RO_0001025 rdf:resource="http://purl.obolibrary.org/obo/GAZ_00000525"/>
        <obo:IAO_0000115>A municipality in the Guatemalan Department of Sacatepequez.</obo:IAO_0000115>
        <oboInOwl:hasOBONamespace>GAZ</oboInOwl:hasOBONamespace>
        <oboInOwl:id>GAZ:00068234</oboInOwl:id>
        <rdfs:label>Municipality of Santa Catarina Barahona</rdfs:label>
    </owl:NamedIndividual>
    


    <!-- http://purl.obolibrary.org/obo/GAZ_00068235 -->

    <owl:NamedIndividual rdf:about="http://purl.obolibrary.org/obo/GAZ_00068235">
        <rdf:type rdf:resource="http://purl.obolibrary.org/obo/ENVO_00000856"/>
        <obo:RO_0001025 rdf:resource="http://purl.obolibrary.org/obo/GAZ_00000525"/>
        <obo:IAO_0000115>A municipality in the Guatemalan Department of Sacatepequez.</obo:IAO_0000115>
        <oboInOwl:hasOBONamespace>GAZ</oboInOwl:hasOBONamespace>
        <oboInOwl:id>GAZ:00068235</oboInOwl:id>
        <rdfs:label>Municipality of Sumpango</rdfs:label>
    </owl:NamedIndividual>
    


    <!-- http://purl.obolibrary.org/obo/GAZ_00068236 -->

    <owl:NamedIndividual rdf:about="http://purl.obolibrary.org/obo/GAZ_00068236">
        <rdf:type rdf:resource="http://purl.obolibrary.org/obo/ENVO_00000856"/>
        <obo:RO_0001025 rdf:resource="http://purl.obolibrary.org/obo/GAZ_00000525"/>
        <obo:IAO_0000115>A municipality in the Guatemalan Department of Sacatepequez.</obo:IAO_0000115>
        <oboInOwl:hasOBONamespace>GAZ</oboInOwl:hasOBONamespace>
        <oboInOwl:id>GAZ:00068236</oboInOwl:id>
        <rdfs:label>Municipality of Ciudad Vieja</rdfs:label>
    </owl:NamedIndividual>
    


    <!-- http://purl.obolibrary.org/obo/GAZ_00068237 -->

    <owl:NamedIndividual rdf:about="http://purl.obolibrary.org/obo/GAZ_00068237">
        <rdf:type rdf:resource="http://purl.obolibrary.org/obo/ENVO_00000856"/>
        <obo:RO_0001025 rdf:resource="http://purl.obolibrary.org/obo/GAZ_00000525"/>
        <obo:IAO_0000115>A municipality in the Guatemalan Department of Sacatepequez.</obo:IAO_0000115>
        <oboInOwl:hasOBONamespace>GAZ</oboInOwl:hasOBONamespace>
        <oboInOwl:id>GAZ:00068237</oboInOwl:id>
        <rdfs:label>Municipality of Santo Domingo Xenacoj</rdfs:label>
    </owl:NamedIndividual>
    


    <!-- http://purl.obolibrary.org/obo/GAZ_00068238 -->

    <owl:NamedIndividual rdf:about="http://purl.obolibrary.org/obo/GAZ_00068238">
        <rdf:type rdf:resource="http://purl.obolibrary.org/obo/ENVO_00000856"/>
        <obo:RO_0001025 rdf:resource="http://purl.obolibrary.org/obo/GAZ_00000525"/>
        <obo:IAO_0000115>A municipality in the Guatemalan Department of Sacatepequez.</obo:IAO_0000115>
        <oboInOwl:hasOBONamespace>GAZ</oboInOwl:hasOBONamespace>
        <oboInOwl:id>GAZ:00068238</oboInOwl:id>
        <rdfs:label>Municipality of San Miguel Duenas</rdfs:label>
    </owl:NamedIndividual>
    


    <!-- http://purl.obolibrary.org/obo/GAZ_00068239 -->

    <owl:NamedIndividual rdf:about="http://purl.obolibrary.org/obo/GAZ_00068239">
        <rdf:type rdf:resource="http://purl.obolibrary.org/obo/ENVO_00000856"/>
        <obo:RO_0001025 rdf:resource="http://purl.obolibrary.org/obo/GAZ_00000525"/>
        <obo:IAO_0000115>A municipality in the Guatemalan Department of Sacatepequez.</obo:IAO_0000115>
        <oboInOwl:hasOBONamespace>GAZ</oboInOwl:hasOBONamespace>
        <oboInOwl:id>GAZ:00068239</oboInOwl:id>
        <rdfs:label>Municipality of Santa Lucia Milpas Altas</rdfs:label>
    </owl:NamedIndividual>
    


    <!-- http://purl.obolibrary.org/obo/GAZ_00068240 -->

    <owl:NamedIndividual rdf:about="http://purl.obolibrary.org/obo/GAZ_00068240">
        <rdf:type rdf:resource="http://purl.obolibrary.org/obo/ENVO_00000856"/>
        <obo:RO_0001025 rdf:resource="http://purl.obolibrary.org/obo/GAZ_00000525"/>
        <obo:IAO_0000115>A municipality in the Guatemalan Department of Sacatepequez.</obo:IAO_0000115>
        <oboInOwl:hasOBONamespace>GAZ</oboInOwl:hasOBONamespace>
        <oboInOwl:id>GAZ:00068240</oboInOwl:id>
        <rdfs:label>Municipality of San Lucas Sacatepequez</rdfs:label>
    </owl:NamedIndividual>
    


    <!-- http://purl.obolibrary.org/obo/GAZ_00068241 -->

    <owl:NamedIndividual rdf:about="http://purl.obolibrary.org/obo/GAZ_00068241">
        <rdf:type rdf:resource="http://purl.obolibrary.org/obo/ENVO_00000856"/>
        <obo:RO_0001025 rdf:resource="http://purl.obolibrary.org/obo/GAZ_00000525"/>
        <obo:IAO_0000115>A municipality in the Guatemalan Department of Sacatepequez.</obo:IAO_0000115>
        <oboInOwl:hasOBONamespace>GAZ</oboInOwl:hasOBONamespace>
        <oboInOwl:id>GAZ:00068241</oboInOwl:id>
        <rdfs:label>Municipality of Santiago Sacatepequez</rdfs:label>
    </owl:NamedIndividual>
    


    <!-- http://purl.obolibrary.org/obo/GAZ_00068242 -->

    <owl:NamedIndividual rdf:about="http://purl.obolibrary.org/obo/GAZ_00068242">
        <rdf:type rdf:resource="http://purl.obolibrary.org/obo/ENVO_00000856"/>
        <obo:RO_0001025 rdf:resource="http://purl.obolibrary.org/obo/GAZ_00000525"/>
        <obo:IAO_0000115>A municipality in the Guatemalan Department of Sacatepequez.</obo:IAO_0000115>
        <oboInOwl:hasOBONamespace>GAZ</oboInOwl:hasOBONamespace>
        <oboInOwl:id>GAZ:00068242</oboInOwl:id>
        <rdfs:label>Municipality of San Bartolome Milpas Altas</rdfs:label>
    </owl:NamedIndividual>
    


    <!-- http://purl.obolibrary.org/obo/GAZ_00068243 -->

    <owl:NamedIndividual rdf:about="http://purl.obolibrary.org/obo/GAZ_00068243">
        <rdf:type rdf:resource="http://purl.obolibrary.org/obo/ENVO_00000856"/>
        <obo:RO_0001025 rdf:resource="http://purl.obolibrary.org/obo/GAZ_00000525"/>
        <obo:IAO_0000115>A municipality in the Guatemalan Department of Sacatepequez.</obo:IAO_0000115>
        <oboInOwl:hasOBONamespace>GAZ</oboInOwl:hasOBONamespace>
        <oboInOwl:id>GAZ:00068243</oboInOwl:id>
        <rdfs:label>Municipality of Santa Maria de Jesus</rdfs:label>
    </owl:NamedIndividual>
    


    <!-- http://purl.obolibrary.org/obo/GAZ_00068244 -->

    <owl:NamedIndividual rdf:about="http://purl.obolibrary.org/obo/GAZ_00068244">
        <rdf:type rdf:resource="http://purl.obolibrary.org/obo/ENVO_00000856"/>
        <obo:RO_0001025 rdf:resource="http://purl.obolibrary.org/obo/GAZ_00000525"/>
        <obo:IAO_0000115>A municipality in the Guatemalan Department of Sacatepequez.</obo:IAO_0000115>
        <oboInOwl:hasOBONamespace>GAZ</oboInOwl:hasOBONamespace>
        <oboInOwl:id>GAZ:00068244</oboInOwl:id>
        <rdfs:label>Municipality of San Antonio Aguas Calientes</rdfs:label>
    </owl:NamedIndividual>
    


    <!-- http://purl.obolibrary.org/obo/GAZ_00068245 -->

    <owl:NamedIndividual rdf:about="http://purl.obolibrary.org/obo/GAZ_00068245">
        <rdf:type rdf:resource="http://purl.obolibrary.org/obo/ENVO_00000856"/>
        <obo:RO_0001025 rdf:resource="http://purl.obolibrary.org/obo/GAZ_00000525"/>
        <obo:IAO_0000115>A municipality in the Guatemalan Department of Sacatepequez.</obo:IAO_0000115>
        <oboInOwl:hasOBONamespace>GAZ</oboInOwl:hasOBONamespace>
        <oboInOwl:id>GAZ:00068245</oboInOwl:id>
        <rdfs:label>Municipality of Antigua Guatemala</rdfs:label>
    </owl:NamedIndividual>
    


    <!-- http://purl.obolibrary.org/obo/GAZ_00068246 -->

    <owl:NamedIndividual rdf:about="http://purl.obolibrary.org/obo/GAZ_00068246">
        <rdf:type rdf:resource="http://purl.obolibrary.org/obo/ENVO_00000856"/>
        <obo:RO_0001025 rdf:resource="http://purl.obolibrary.org/obo/GAZ_00000529"/>
        <obo:IAO_0000115>A municipality in the San Marcos Department of Guatemala.</obo:IAO_0000115>
        <oboInOwl:hasOBONamespace>GAZ</oboInOwl:hasOBONamespace>
        <oboInOwl:id>GAZ:00068246</oboInOwl:id>
        <rdfs:label>Municipality of El Quetzal</rdfs:label>
    </owl:NamedIndividual>
    


    <!-- http://purl.obolibrary.org/obo/GAZ_00068247 -->

    <owl:NamedIndividual rdf:about="http://purl.obolibrary.org/obo/GAZ_00068247">
        <rdf:type rdf:resource="http://purl.obolibrary.org/obo/ENVO_00000856"/>
        <obo:RO_0001025 rdf:resource="http://purl.obolibrary.org/obo/GAZ_00000529"/>
        <obo:IAO_0000115>A municipality in the San Marcos Department of Guatemala.</obo:IAO_0000115>
        <oboInOwl:hasOBONamespace>GAZ</oboInOwl:hasOBONamespace>
        <oboInOwl:id>GAZ:00068247</oboInOwl:id>
        <rdfs:label>Municipality of Catarina</rdfs:label>
    </owl:NamedIndividual>
    


    <!-- http://purl.obolibrary.org/obo/GAZ_00068248 -->

    <owl:NamedIndividual rdf:about="http://purl.obolibrary.org/obo/GAZ_00068248">
        <rdf:type rdf:resource="http://purl.obolibrary.org/obo/ENVO_00000856"/>
        <obo:RO_0001025 rdf:resource="http://purl.obolibrary.org/obo/GAZ_00000529"/>
        <obo:IAO_0000115>A municipality in the San Marcos Department of Guatemala.</obo:IAO_0000115>
        <oboInOwl:hasOBONamespace>GAZ</oboInOwl:hasOBONamespace>
        <oboInOwl:id>GAZ:00068248</oboInOwl:id>
        <rdfs:label>Municipality of San Miguel Ixtahuacan</rdfs:label>
    </owl:NamedIndividual>
    


    <!-- http://purl.obolibrary.org/obo/GAZ_00068249 -->

    <owl:NamedIndividual rdf:about="http://purl.obolibrary.org/obo/GAZ_00068249">
        <rdf:type rdf:resource="http://purl.obolibrary.org/obo/ENVO_00000856"/>
        <obo:RO_0001025 rdf:resource="http://purl.obolibrary.org/obo/GAZ_00000529"/>
        <obo:IAO_0000115>A municipality in the San Marcos Department of Guatemala.</obo:IAO_0000115>
        <oboInOwl:hasOBONamespace>GAZ</oboInOwl:hasOBONamespace>
        <oboInOwl:id>GAZ:00068249</oboInOwl:id>
        <rdfs:label>Municipality of Concepcion Tutuapa</rdfs:label>
    </owl:NamedIndividual>
    


    <!-- http://purl.obolibrary.org/obo/GAZ_00068250 -->

    <owl:NamedIndividual rdf:about="http://purl.obolibrary.org/obo/GAZ_00068250">
        <rdf:type rdf:resource="http://purl.obolibrary.org/obo/ENVO_00000856"/>
        <obo:RO_0001025 rdf:resource="http://purl.obolibrary.org/obo/GAZ_00000529"/>
        <obo:IAO_0000115>A municipality in the San Marcos Department of Guatemala.</obo:IAO_0000115>
        <oboInOwl:hasOBONamespace>GAZ</oboInOwl:hasOBONamespace>
        <oboInOwl:id>GAZ:00068250</oboInOwl:id>
        <rdfs:label>Municipality of Pajapita</rdfs:label>
    </owl:NamedIndividual>
    


    <!-- http://purl.obolibrary.org/obo/GAZ_00068251 -->

    <owl:NamedIndividual rdf:about="http://purl.obolibrary.org/obo/GAZ_00068251">
        <rdf:type rdf:resource="http://purl.obolibrary.org/obo/ENVO_00000856"/>
        <obo:RO_0001025 rdf:resource="http://purl.obolibrary.org/obo/GAZ_00000529"/>
        <obo:IAO_0000115>A municipality in the San Marcos Department of Guatemala.</obo:IAO_0000115>
        <oboInOwl:hasOBONamespace>GAZ</oboInOwl:hasOBONamespace>
        <oboInOwl:id>GAZ:00068251</oboInOwl:id>
        <rdfs:label>Municipality of San Marcos</rdfs:label>
    </owl:NamedIndividual>
    


    <!-- http://purl.obolibrary.org/obo/GAZ_00068252 -->

    <owl:NamedIndividual rdf:about="http://purl.obolibrary.org/obo/GAZ_00068252">
        <rdf:type rdf:resource="http://purl.obolibrary.org/obo/ENVO_00000856"/>
        <obo:RO_0001025 rdf:resource="http://purl.obolibrary.org/obo/GAZ_00000529"/>
        <obo:IAO_0000115>A municipality in the San Marcos Department of Guatemala.</obo:IAO_0000115>
        <oboInOwl:hasOBONamespace>GAZ</oboInOwl:hasOBONamespace>
        <oboInOwl:id>GAZ:00068252</oboInOwl:id>
        <rdfs:label>Municipality of San Rafael Pie de la Cuesta</rdfs:label>
    </owl:NamedIndividual>
    


    <!-- http://purl.obolibrary.org/obo/GAZ_00068253 -->

    <owl:NamedIndividual rdf:about="http://purl.obolibrary.org/obo/GAZ_00068253">
        <rdf:type rdf:resource="http://purl.obolibrary.org/obo/ENVO_00000856"/>
        <obo:RO_0001025 rdf:resource="http://purl.obolibrary.org/obo/GAZ_00000529"/>
        <obo:IAO_0000115>A municipality in the San Marcos Department of Guatemala.</obo:IAO_0000115>
        <oboInOwl:hasOBONamespace>GAZ</oboInOwl:hasOBONamespace>
        <oboInOwl:id>GAZ:00068253</oboInOwl:id>
        <rdfs:label>Municipality of El Rodeo</rdfs:label>
    </owl:NamedIndividual>
    


    <!-- http://purl.obolibrary.org/obo/GAZ_00068254 -->

    <owl:NamedIndividual rdf:about="http://purl.obolibrary.org/obo/GAZ_00068254">
        <rdf:type rdf:resource="http://purl.obolibrary.org/obo/ENVO_00000856"/>
        <obo:RO_0001025 rdf:resource="http://purl.obolibrary.org/obo/GAZ_00000529"/>
        <obo:IAO_0000115>A municipality in the San Marcos Department of Guatemala.</obo:IAO_0000115>
        <oboInOwl:hasOBONamespace>GAZ</oboInOwl:hasOBONamespace>
        <oboInOwl:id>GAZ:00068254</oboInOwl:id>
        <rdfs:label>Municipality of Tajumulco</rdfs:label>
    </owl:NamedIndividual>
    


    <!-- http://purl.obolibrary.org/obo/GAZ_00068255 -->

    <owl:NamedIndividual rdf:about="http://purl.obolibrary.org/obo/GAZ_00068255">
        <rdf:type rdf:resource="http://purl.obolibrary.org/obo/ENVO_00000856"/>
        <obo:RO_0001025 rdf:resource="http://purl.obolibrary.org/obo/GAZ_00000529"/>
        <obo:IAO_0000115>A municipality in the San Marcos Department of Guatemala.</obo:IAO_0000115>
        <oboInOwl:hasOBONamespace>GAZ</oboInOwl:hasOBONamespace>
        <oboInOwl:id>GAZ:00068255</oboInOwl:id>
        <rdfs:label>Municipality of San Pablo</rdfs:label>
    </owl:NamedIndividual>
    


    <!-- http://purl.obolibrary.org/obo/GAZ_00068256 -->

    <owl:NamedIndividual rdf:about="http://purl.obolibrary.org/obo/GAZ_00068256">
        <rdf:type rdf:resource="http://purl.obolibrary.org/obo/ENVO_00000856"/>
        <obo:RO_0001025 rdf:resource="http://purl.obolibrary.org/obo/GAZ_00000529"/>
        <obo:IAO_0000115>A municipality in the San Marcos Department of Guatemala.</obo:IAO_0000115>
        <oboInOwl:hasOBONamespace>GAZ</oboInOwl:hasOBONamespace>
        <oboInOwl:id>GAZ:00068256</oboInOwl:id>
        <rdfs:label>Municipality of Sipacapa</rdfs:label>
    </owl:NamedIndividual>
    


    <!-- http://purl.obolibrary.org/obo/GAZ_00068257 -->

    <owl:NamedIndividual rdf:about="http://purl.obolibrary.org/obo/GAZ_00068257">
        <rdf:type rdf:resource="http://purl.obolibrary.org/obo/ENVO_00000856"/>
        <obo:RO_0001025 rdf:resource="http://purl.obolibrary.org/obo/GAZ_00000529"/>
        <obo:IAO_0000115>A municipality in the San Marcos Department of Guatemala.</obo:IAO_0000115>
        <oboInOwl:hasOBONamespace>GAZ</oboInOwl:hasOBONamespace>
        <oboInOwl:id>GAZ:00068257</oboInOwl:id>
        <rdfs:label>Municipality of Ayutla</rdfs:label>
    </owl:NamedIndividual>
    


    <!-- http://purl.obolibrary.org/obo/GAZ_00068258 -->

    <owl:NamedIndividual rdf:about="http://purl.obolibrary.org/obo/GAZ_00068258">
        <rdf:type rdf:resource="http://purl.obolibrary.org/obo/ENVO_00000856"/>
        <obo:RO_0001025 rdf:resource="http://purl.obolibrary.org/obo/GAZ_00000529"/>
        <obo:IAO_0000115>A municipality in the San Marcos Department of Guatemala.</obo:IAO_0000115>
        <oboInOwl:hasOBONamespace>GAZ</oboInOwl:hasOBONamespace>
        <oboInOwl:id>GAZ:00068258</oboInOwl:id>
        <rdfs:label>Municipality of El Tumbador</rdfs:label>
    </owl:NamedIndividual>
    


    <!-- http://purl.obolibrary.org/obo/GAZ_00068259 -->

    <owl:NamedIndividual rdf:about="http://purl.obolibrary.org/obo/GAZ_00068259">
        <rdf:type rdf:resource="http://purl.obolibrary.org/obo/ENVO_00000856"/>
        <obo:RO_0001025 rdf:resource="http://purl.obolibrary.org/obo/GAZ_00000529"/>
        <obo:IAO_0000115>A municipality in the San Marcos Department of Guatemala.</obo:IAO_0000115>
        <oboInOwl:hasOBONamespace>GAZ</oboInOwl:hasOBONamespace>
        <oboInOwl:id>GAZ:00068259</oboInOwl:id>
        <rdfs:label>Municipality of Sibinal</rdfs:label>
    </owl:NamedIndividual>
    


    <!-- http://purl.obolibrary.org/obo/GAZ_00068260 -->

    <owl:NamedIndividual rdf:about="http://purl.obolibrary.org/obo/GAZ_00068260">
        <rdf:type rdf:resource="http://purl.obolibrary.org/obo/ENVO_00000856"/>
        <obo:RO_0001025 rdf:resource="http://purl.obolibrary.org/obo/GAZ_00000529"/>
        <obo:IAO_0000115>A municipality in the San Marcos Department of Guatemala.</obo:IAO_0000115>
        <oboInOwl:hasOBONamespace>GAZ</oboInOwl:hasOBONamespace>
        <oboInOwl:id>GAZ:00068260</oboInOwl:id>
        <rdfs:label>Municipality of Tacana</rdfs:label>
    </owl:NamedIndividual>
    


    <!-- http://purl.obolibrary.org/obo/GAZ_00068261 -->

    <owl:NamedIndividual rdf:about="http://purl.obolibrary.org/obo/GAZ_00068261">
        <rdf:type rdf:resource="http://purl.obolibrary.org/obo/ENVO_00000856"/>
        <obo:RO_0001025 rdf:resource="http://purl.obolibrary.org/obo/GAZ_00000529"/>
        <obo:IAO_0000115>A municipality in the San Marcos Department of Guatemala.</obo:IAO_0000115>
        <oboInOwl:hasOBONamespace>GAZ</oboInOwl:hasOBONamespace>
        <oboInOwl:id>GAZ:00068261</oboInOwl:id>
        <rdfs:label>Municipality of Nuevo Progreso</rdfs:label>
    </owl:NamedIndividual>
    


    <!-- http://purl.obolibrary.org/obo/GAZ_00068262 -->

    <owl:NamedIndividual rdf:about="http://purl.obolibrary.org/obo/GAZ_00068262">
        <rdf:type rdf:resource="http://purl.obolibrary.org/obo/ENVO_00000856"/>
        <obo:RO_0001025 rdf:resource="http://purl.obolibrary.org/obo/GAZ_00000529"/>
        <obo:IAO_0000115>A municipality in the San Marcos Department of Guatemala.</obo:IAO_0000115>
        <oboInOwl:hasOBONamespace>GAZ</oboInOwl:hasOBONamespace>
        <oboInOwl:id>GAZ:00068262</oboInOwl:id>
        <rdfs:label>Municipality of Rio Blanco</rdfs:label>
    </owl:NamedIndividual>
    


    <!-- http://purl.obolibrary.org/obo/GAZ_00068263 -->

    <owl:NamedIndividual rdf:about="http://purl.obolibrary.org/obo/GAZ_00068263">
        <rdf:type rdf:resource="http://purl.obolibrary.org/obo/ENVO_00000856"/>
        <obo:RO_0001025 rdf:resource="http://purl.obolibrary.org/obo/GAZ_00000529"/>
        <obo:IAO_0000115>A municipality in the San Marcos Department of Guatemala.</obo:IAO_0000115>
        <oboInOwl:hasOBONamespace>GAZ</oboInOwl:hasOBONamespace>
        <oboInOwl:id>GAZ:00068263</oboInOwl:id>
        <rdfs:label>Municipality of San Antonio Sacatepequez</rdfs:label>
    </owl:NamedIndividual>
    


    <!-- http://purl.obolibrary.org/obo/GAZ_00068264 -->

    <owl:NamedIndividual rdf:about="http://purl.obolibrary.org/obo/GAZ_00068264">
        <rdf:type rdf:resource="http://purl.obolibrary.org/obo/ENVO_00000856"/>
        <obo:RO_0001025 rdf:resource="http://purl.obolibrary.org/obo/GAZ_00000529"/>
        <obo:IAO_0000115>A municipality in the San Marcos Department of Guatemala.</obo:IAO_0000115>
        <oboInOwl:hasOBONamespace>GAZ</oboInOwl:hasOBONamespace>
        <oboInOwl:id>GAZ:00068264</oboInOwl:id>
        <rdfs:label>Municipality of San Lorenzo</rdfs:label>
    </owl:NamedIndividual>
    


    <!-- http://purl.obolibrary.org/obo/GAZ_00068265 -->

    <owl:NamedIndividual rdf:about="http://purl.obolibrary.org/obo/GAZ_00068265">
        <rdf:type rdf:resource="http://purl.obolibrary.org/obo/ENVO_00000856"/>
        <obo:RO_0001025 rdf:resource="http://purl.obolibrary.org/obo/GAZ_00000529"/>
        <obo:IAO_0000115>A municipality in the San Marcos Department of Guatemala.</obo:IAO_0000115>
        <oboInOwl:hasOBONamespace>GAZ</oboInOwl:hasOBONamespace>
        <oboInOwl:id>GAZ:00068265</oboInOwl:id>
        <rdfs:label>Municipality of Malacatan</rdfs:label>
    </owl:NamedIndividual>
    


    <!-- http://purl.obolibrary.org/obo/GAZ_00068266 -->

    <owl:NamedIndividual rdf:about="http://purl.obolibrary.org/obo/GAZ_00068266">
        <rdf:type rdf:resource="http://purl.obolibrary.org/obo/ENVO_00000856"/>
        <obo:RO_0001025 rdf:resource="http://purl.obolibrary.org/obo/GAZ_00000529"/>
        <obo:IAO_0000115>A municipality in the San Marcos Department of Guatemala.</obo:IAO_0000115>
        <oboInOwl:hasOBONamespace>GAZ</oboInOwl:hasOBONamespace>
        <oboInOwl:id>GAZ:00068266</oboInOwl:id>
        <rdfs:label>Municipality of San Cristobal Cucho</rdfs:label>
    </owl:NamedIndividual>
    


    <!-- http://purl.obolibrary.org/obo/GAZ_00068267 -->

    <owl:NamedIndividual rdf:about="http://purl.obolibrary.org/obo/GAZ_00068267">
        <rdf:type rdf:resource="http://purl.obolibrary.org/obo/ENVO_00000856"/>
        <obo:RO_0001025 rdf:resource="http://purl.obolibrary.org/obo/GAZ_00000529"/>
        <obo:IAO_0000115>A municipality in the San Marcos Department of Guatemala.</obo:IAO_0000115>
        <oboInOwl:hasOBONamespace>GAZ</oboInOwl:hasOBONamespace>
        <oboInOwl:id>GAZ:00068267</oboInOwl:id>
        <rdfs:label>Municipality of San Jose Ojetenam</rdfs:label>
    </owl:NamedIndividual>
    


    <!-- http://purl.obolibrary.org/obo/GAZ_00068268 -->

    <owl:NamedIndividual rdf:about="http://purl.obolibrary.org/obo/GAZ_00068268">
        <rdf:type rdf:resource="http://purl.obolibrary.org/obo/ENVO_00000856"/>
        <obo:RO_0001025 rdf:resource="http://purl.obolibrary.org/obo/GAZ_00000529"/>
        <obo:IAO_0000115>A municipality in the San Marcos Department of Guatemala.</obo:IAO_0000115>
        <oboInOwl:hasOBONamespace>GAZ</oboInOwl:hasOBONamespace>
        <oboInOwl:id>GAZ:00068268</oboInOwl:id>
        <rdfs:label>Municipality of Ocos</rdfs:label>
    </owl:NamedIndividual>
    


    <!-- http://purl.obolibrary.org/obo/GAZ_00068269 -->

    <owl:NamedIndividual rdf:about="http://purl.obolibrary.org/obo/GAZ_00068269">
        <rdf:type rdf:resource="http://purl.obolibrary.org/obo/ENVO_00000856"/>
        <obo:RO_0001025 rdf:resource="http://purl.obolibrary.org/obo/GAZ_00000529"/>
        <obo:IAO_0000115>A municipality in the San Marcos Department of Guatemala.</obo:IAO_0000115>
        <oboInOwl:hasOBONamespace>GAZ</oboInOwl:hasOBONamespace>
        <oboInOwl:id>GAZ:00068269</oboInOwl:id>
        <rdfs:label>Municipality of Ixchiguan</rdfs:label>
    </owl:NamedIndividual>
    


    <!-- http://purl.obolibrary.org/obo/GAZ_00068270 -->

    <owl:NamedIndividual rdf:about="http://purl.obolibrary.org/obo/GAZ_00068270">
        <rdf:type rdf:resource="http://purl.obolibrary.org/obo/ENVO_00000856"/>
        <obo:RO_0001025 rdf:resource="http://purl.obolibrary.org/obo/GAZ_00000529"/>
        <obo:IAO_0000115>A municipality in the San Marcos Department of Guatemala.</obo:IAO_0000115>
        <oboInOwl:hasOBONamespace>GAZ</oboInOwl:hasOBONamespace>
        <oboInOwl:id>GAZ:00068270</oboInOwl:id>
        <rdfs:label>Municipality of La Reforma</rdfs:label>
    </owl:NamedIndividual>
    


    <!-- http://purl.obolibrary.org/obo/GAZ_00068271 -->

    <owl:NamedIndividual rdf:about="http://purl.obolibrary.org/obo/GAZ_00068271">
        <rdf:type rdf:resource="http://purl.obolibrary.org/obo/ENVO_00000856"/>
        <obo:RO_0001025 rdf:resource="http://purl.obolibrary.org/obo/GAZ_00000540"/>
        <obo:IAO_0000115>A municipality in Santa Rosa Department of Guatemala.</obo:IAO_0000115>
        <oboInOwl:hasOBONamespace>GAZ</oboInOwl:hasOBONamespace>
        <oboInOwl:id>GAZ:00068271</oboInOwl:id>
        <rdfs:label>Municipality of Casillas</rdfs:label>
    </owl:NamedIndividual>
    


    <!-- http://purl.obolibrary.org/obo/GAZ_00068272 -->

    <owl:NamedIndividual rdf:about="http://purl.obolibrary.org/obo/GAZ_00068272">
        <rdf:type rdf:resource="http://purl.obolibrary.org/obo/ENVO_00000856"/>
        <obo:RO_0001025 rdf:resource="http://purl.obolibrary.org/obo/GAZ_00000540"/>
        <obo:IAO_0000115>A municipality in the Santa Rosa Department of Guatemala.</obo:IAO_0000115>
        <oboInOwl:hasOBONamespace>GAZ</oboInOwl:hasOBONamespace>
        <oboInOwl:id>GAZ:00068272</oboInOwl:id>
        <rdfs:label>Municipality of Taxisco</rdfs:label>
    </owl:NamedIndividual>
    


    <!-- http://purl.obolibrary.org/obo/GAZ_00068273 -->

    <owl:NamedIndividual rdf:about="http://purl.obolibrary.org/obo/GAZ_00068273">
        <rdf:type rdf:resource="http://purl.obolibrary.org/obo/ENVO_00000856"/>
        <obo:RO_0001025 rdf:resource="http://purl.obolibrary.org/obo/GAZ_00000541"/>
        <obo:IAO_0000115>A municipality in the Solola Department of Guatemala.</obo:IAO_0000115>
        <oboInOwl:hasOBONamespace>GAZ</oboInOwl:hasOBONamespace>
        <oboInOwl:id>GAZ:00068273</oboInOwl:id>
        <rdfs:label>Municipality of San Antonio Palopo</rdfs:label>
    </owl:NamedIndividual>
    


    <!-- http://purl.obolibrary.org/obo/GAZ_00068274 -->

    <owl:NamedIndividual rdf:about="http://purl.obolibrary.org/obo/GAZ_00068274">
        <rdf:type rdf:resource="http://purl.obolibrary.org/obo/ENVO_00000856"/>
        <obo:RO_0001025 rdf:resource="http://purl.obolibrary.org/obo/GAZ_00000540"/>
        <obo:IAO_0000115>A municipality in Santa Rosa Department of Guatemala.</obo:IAO_0000115>
        <oboInOwl:hasOBONamespace>GAZ</oboInOwl:hasOBONamespace>
        <oboInOwl:id>GAZ:00068274</oboInOwl:id>
        <rdfs:label>Municipality of Barberena</rdfs:label>
    </owl:NamedIndividual>
    


    <!-- http://purl.obolibrary.org/obo/GAZ_00068275 -->

    <owl:NamedIndividual rdf:about="http://purl.obolibrary.org/obo/GAZ_00068275">
        <rdf:type rdf:resource="http://purl.obolibrary.org/obo/ENVO_00000856"/>
        <obo:RO_0001025 rdf:resource="http://purl.obolibrary.org/obo/GAZ_00000540"/>
        <obo:IAO_0000115>A municipality in Santa Rosa Department of Guatemala.</obo:IAO_0000115>
        <oboInOwl:hasOBONamespace>GAZ</oboInOwl:hasOBONamespace>
        <oboInOwl:id>GAZ:00068275</oboInOwl:id>
        <rdfs:label>Municipality of Nueva Santa Rosa</rdfs:label>
    </owl:NamedIndividual>
    


    <!-- http://purl.obolibrary.org/obo/GAZ_00068276 -->

    <owl:NamedIndividual rdf:about="http://purl.obolibrary.org/obo/GAZ_00068276">
        <rdf:type rdf:resource="http://purl.obolibrary.org/obo/ENVO_00000856"/>
        <obo:RO_0001025 rdf:resource="http://purl.obolibrary.org/obo/GAZ_00000540"/>
        <obo:IAO_0000115>A municipality in Santa Rosa Department of Guatemala.</obo:IAO_0000115>
        <oboInOwl:hasOBONamespace>GAZ</oboInOwl:hasOBONamespace>
        <oboInOwl:id>GAZ:00068276</oboInOwl:id>
        <rdfs:label>Municipality of Santa Rosa Cuilapa</rdfs:label>
    </owl:NamedIndividual>
    


    <!-- http://purl.obolibrary.org/obo/GAZ_00068277 -->

    <owl:NamedIndividual rdf:about="http://purl.obolibrary.org/obo/GAZ_00068277">
        <rdf:type rdf:resource="http://purl.obolibrary.org/obo/ENVO_00000856"/>
        <obo:RO_0001025 rdf:resource="http://purl.obolibrary.org/obo/GAZ_00000540"/>
        <obo:IAO_0000115>A municipality in Santa Rosa Department of Guatemala.</obo:IAO_0000115>
        <oboInOwl:hasOBONamespace>GAZ</oboInOwl:hasOBONamespace>
        <oboInOwl:id>GAZ:00068277</oboInOwl:id>
        <rdfs:label>Municipality of Oratorio</rdfs:label>
    </owl:NamedIndividual>
    


    <!-- http://purl.obolibrary.org/obo/GAZ_00068278 -->

    <owl:NamedIndividual rdf:about="http://purl.obolibrary.org/obo/GAZ_00068278">
        <rdf:type rdf:resource="http://purl.obolibrary.org/obo/ENVO_00000856"/>
        <obo:RO_0001025 rdf:resource="http://purl.obolibrary.org/obo/GAZ_00000541"/>
        <obo:IAO_0000115>A municipality in the Solola Department of Guatemala.</obo:IAO_0000115>
        <oboInOwl:hasOBONamespace>GAZ</oboInOwl:hasOBONamespace>
        <oboInOwl:id>GAZ:00068278</oboInOwl:id>
        <rdfs:label>Municipality of San Andres Semetabaj</rdfs:label>
    </owl:NamedIndividual>
    


    <!-- http://purl.obolibrary.org/obo/GAZ_00068279 -->

    <owl:NamedIndividual rdf:about="http://purl.obolibrary.org/obo/GAZ_00068279">
        <rdf:type rdf:resource="http://purl.obolibrary.org/obo/ENVO_00000856"/>
        <obo:RO_0001025 rdf:resource="http://purl.obolibrary.org/obo/GAZ_00000540"/>
        <obo:IAO_0000115>A municipality in Santa Rosa Department of Guatemala.</obo:IAO_0000115>
        <oboInOwl:hasOBONamespace>GAZ</oboInOwl:hasOBONamespace>
        <oboInOwl:id>GAZ:00068279</oboInOwl:id>
        <rdfs:label>Municipality of Pueblo Nuevo Vinas</rdfs:label>
    </owl:NamedIndividual>
    


    <!-- http://purl.obolibrary.org/obo/GAZ_00068280 -->

    <owl:NamedIndividual rdf:about="http://purl.obolibrary.org/obo/GAZ_00068280">
        <rdf:type rdf:resource="http://purl.obolibrary.org/obo/ENVO_00000856"/>
        <obo:RO_0001025 rdf:resource="http://purl.obolibrary.org/obo/GAZ_00000540"/>
        <obo:IAO_0000115>A municipality in Santa Rosa Department of Guatemala.</obo:IAO_0000115>
        <oboInOwl:hasOBONamespace>GAZ</oboInOwl:hasOBONamespace>
        <oboInOwl:id>GAZ:00068280</oboInOwl:id>
        <rdfs:label>Municipality of Guazacapan</rdfs:label>
    </owl:NamedIndividual>
    


    <!-- http://purl.obolibrary.org/obo/GAZ_00068281 -->

    <owl:NamedIndividual rdf:about="http://purl.obolibrary.org/obo/GAZ_00068281">
        <rdf:type rdf:resource="http://purl.obolibrary.org/obo/ENVO_00000856"/>
        <obo:RO_0001025 rdf:resource="http://purl.obolibrary.org/obo/GAZ_00000540"/>
        <obo:IAO_0000115>A municipality in Santa Rosa Department of Guatemala.</obo:IAO_0000115>
        <oboInOwl:hasOBONamespace>GAZ</oboInOwl:hasOBONamespace>
        <oboInOwl:id>GAZ:00068281</oboInOwl:id>
        <rdfs:label>Municipality of San Juan Tecuaco</rdfs:label>
    </owl:NamedIndividual>
    


    <!-- http://purl.obolibrary.org/obo/GAZ_00068282 -->

    <owl:NamedIndividual rdf:about="http://purl.obolibrary.org/obo/GAZ_00068282">
        <rdf:type rdf:resource="http://purl.obolibrary.org/obo/ENVO_00000856"/>
        <obo:RO_0001025 rdf:resource="http://purl.obolibrary.org/obo/GAZ_00000540"/>
        <obo:IAO_0000115>A municipality in Santa Rosa Department of Guatemala.</obo:IAO_0000115>
        <oboInOwl:hasOBONamespace>GAZ</oboInOwl:hasOBONamespace>
        <oboInOwl:id>GAZ:00068282</oboInOwl:id>
        <rdfs:label>Municipality of Santa Maria Ixhuatan</rdfs:label>
    </owl:NamedIndividual>
    


    <!-- http://purl.obolibrary.org/obo/GAZ_00068283 -->

    <owl:NamedIndividual rdf:about="http://purl.obolibrary.org/obo/GAZ_00068283">
        <rdf:type rdf:resource="http://purl.obolibrary.org/obo/ENVO_00000856"/>
        <obo:RO_0001025 rdf:resource="http://purl.obolibrary.org/obo/GAZ_00000541"/>
        <obo:IAO_0000115>A municipality in the Solola Department of Guatemala.</obo:IAO_0000115>
        <oboInOwl:hasOBONamespace>GAZ</oboInOwl:hasOBONamespace>
        <oboInOwl:id>GAZ:00068283</oboInOwl:id>
        <rdfs:label>Municipality of Santa Clara La Laguna</rdfs:label>
    </owl:NamedIndividual>
    


    <!-- http://purl.obolibrary.org/obo/GAZ_00068284 -->

    <owl:NamedIndividual rdf:about="http://purl.obolibrary.org/obo/GAZ_00068284">
        <rdf:type rdf:resource="http://purl.obolibrary.org/obo/ENVO_00000856"/>
        <obo:RO_0001025 rdf:resource="http://purl.obolibrary.org/obo/GAZ_00000540"/>
        <obo:IAO_0000115>A municipality in Santa Rosa Department of Guatemala.</obo:IAO_0000115>
        <oboInOwl:hasOBONamespace>GAZ</oboInOwl:hasOBONamespace>
        <oboInOwl:id>GAZ:00068284</oboInOwl:id>
        <rdfs:label>Municipality of Santa Cruz Naranjo</rdfs:label>
    </owl:NamedIndividual>
    


    <!-- http://purl.obolibrary.org/obo/GAZ_00068285 -->

    <owl:NamedIndividual rdf:about="http://purl.obolibrary.org/obo/GAZ_00068285">
        <rdf:type rdf:resource="http://purl.obolibrary.org/obo/ENVO_00000856"/>
        <obo:RO_0001025 rdf:resource="http://purl.obolibrary.org/obo/GAZ_00000540"/>
        <obo:IAO_0000115>A municipality in the Santa Rosa Department of Guatemala.</obo:IAO_0000115>
        <oboInOwl:hasOBONamespace>GAZ</oboInOwl:hasOBONamespace>
        <oboInOwl:id>GAZ:00068285</oboInOwl:id>
        <rdfs:label>Municipality of Santa Rosa de Lima</rdfs:label>
    </owl:NamedIndividual>
    


    <!-- http://purl.obolibrary.org/obo/GAZ_00068286 -->

    <owl:NamedIndividual rdf:about="http://purl.obolibrary.org/obo/GAZ_00068286">
        <rdf:type rdf:resource="http://purl.obolibrary.org/obo/ENVO_00000856"/>
        <obo:RO_0001025 rdf:resource="http://purl.obolibrary.org/obo/GAZ_00000540"/>
        <obo:IAO_0000115>A municipality in Santa Rosa Department of Guatemala.</obo:IAO_0000115>
        <oboInOwl:hasOBONamespace>GAZ</oboInOwl:hasOBONamespace>
        <oboInOwl:id>GAZ:00068286</oboInOwl:id>
        <rdfs:label>Municipality of San Rafael Las Flores</rdfs:label>
    </owl:NamedIndividual>
    


    <!-- http://purl.obolibrary.org/obo/GAZ_00068287 -->

    <owl:NamedIndividual rdf:about="http://purl.obolibrary.org/obo/GAZ_00068287">
        <rdf:type rdf:resource="http://purl.obolibrary.org/obo/ENVO_00000856"/>
        <obo:RO_0001025 rdf:resource="http://purl.obolibrary.org/obo/GAZ_00000540"/>
        <obo:IAO_0000115>A municipality in Santa Rosa Department of Guatemala.</obo:IAO_0000115>
        <oboInOwl:hasOBONamespace>GAZ</oboInOwl:hasOBONamespace>
        <oboInOwl:id>GAZ:00068287</oboInOwl:id>
        <rdfs:label>Municipality of Chiquimulilla</rdfs:label>
    </owl:NamedIndividual>
    


    <!-- http://purl.obolibrary.org/obo/GAZ_00068288 -->

    <owl:NamedIndividual rdf:about="http://purl.obolibrary.org/obo/GAZ_00068288">
        <rdf:type rdf:resource="http://purl.obolibrary.org/obo/ENVO_00000856"/>
        <obo:RO_0001025 rdf:resource="http://purl.obolibrary.org/obo/GAZ_00000541"/>
        <obo:IAO_0000115>A municipality in the Solola Department of Guatemala.</obo:IAO_0000115>
        <oboInOwl:hasOBONamespace>GAZ</oboInOwl:hasOBONamespace>
        <oboInOwl:id>GAZ:00068288</oboInOwl:id>
        <rdfs:label>Municipality of Santa Cruz La Laguna</rdfs:label>
    </owl:NamedIndividual>
    


    <!-- http://purl.obolibrary.org/obo/GAZ_00068289 -->

    <owl:NamedIndividual rdf:about="http://purl.obolibrary.org/obo/GAZ_00068289">
        <rdf:type rdf:resource="http://purl.obolibrary.org/obo/ENVO_00000856"/>
        <obo:RO_0001025 rdf:resource="http://purl.obolibrary.org/obo/GAZ_00000541"/>
        <obo:IAO_0000115>A municipality in the Solola Department of Guatemala.</obo:IAO_0000115>
        <oboInOwl:hasOBONamespace>GAZ</oboInOwl:hasOBONamespace>
        <oboInOwl:id>GAZ:00068289</oboInOwl:id>
        <rdfs:label>Municipality of Santa Maria Visitacion</rdfs:label>
    </owl:NamedIndividual>
    


    <!-- http://purl.obolibrary.org/obo/GAZ_00068290 -->

    <owl:NamedIndividual rdf:about="http://purl.obolibrary.org/obo/GAZ_00068290">
        <rdf:type rdf:resource="http://purl.obolibrary.org/obo/ENVO_00000856"/>
        <obo:RO_0001025 rdf:resource="http://purl.obolibrary.org/obo/GAZ_00000541"/>
        <obo:IAO_0000115>A municipality in the Solola Department of Guatemala.</obo:IAO_0000115>
        <oboInOwl:hasOBONamespace>GAZ</oboInOwl:hasOBONamespace>
        <oboInOwl:id>GAZ:00068290</oboInOwl:id>
        <rdfs:label>Municipality of Nahuala</rdfs:label>
    </owl:NamedIndividual>
    


    <!-- http://purl.obolibrary.org/obo/GAZ_00068291 -->

    <owl:NamedIndividual rdf:about="http://purl.obolibrary.org/obo/GAZ_00068291">
        <rdf:type rdf:resource="http://purl.obolibrary.org/obo/ENVO_00000856"/>
        <obo:RO_0001025 rdf:resource="http://purl.obolibrary.org/obo/GAZ_00000541"/>
        <obo:IAO_0000115>A municipality in the Solola Department of Guatemala.</obo:IAO_0000115>
        <oboInOwl:hasOBONamespace>GAZ</oboInOwl:hasOBONamespace>
        <oboInOwl:id>GAZ:00068291</oboInOwl:id>
        <rdfs:label>Municipality of Santa Catarina Ixtahuacan</rdfs:label>
    </owl:NamedIndividual>
    


    <!-- http://purl.obolibrary.org/obo/GAZ_00068292 -->

    <owl:NamedIndividual rdf:about="http://purl.obolibrary.org/obo/GAZ_00068292">
        <rdf:type rdf:resource="http://purl.obolibrary.org/obo/ENVO_00000856"/>
        <obo:RO_0001025 rdf:resource="http://purl.obolibrary.org/obo/GAZ_00000541"/>
        <obo:IAO_0000115>A municipality in the Solola Department of Guatemala.</obo:IAO_0000115>
        <oboInOwl:hasOBONamespace>GAZ</oboInOwl:hasOBONamespace>
        <oboInOwl:id>GAZ:00068292</oboInOwl:id>
        <rdfs:label>Municipality of Concepcion</rdfs:label>
    </owl:NamedIndividual>
    


    <!-- http://purl.obolibrary.org/obo/GAZ_00068293 -->

    <owl:NamedIndividual rdf:about="http://purl.obolibrary.org/obo/GAZ_00068293">
        <rdf:type rdf:resource="http://purl.obolibrary.org/obo/ENVO_00000856"/>
        <obo:RO_0001025 rdf:resource="http://purl.obolibrary.org/obo/GAZ_00000541"/>
        <obo:IAO_0000115>A municipality in the Solola Department of Guatemala.</obo:IAO_0000115>
        <oboInOwl:hasOBONamespace>GAZ</oboInOwl:hasOBONamespace>
        <oboInOwl:id>GAZ:00068293</oboInOwl:id>
        <rdfs:label>Municipality of Santa Lucia Utatlan</rdfs:label>
    </owl:NamedIndividual>
    


    <!-- http://purl.obolibrary.org/obo/GAZ_00068294 -->

    <owl:NamedIndividual rdf:about="http://purl.obolibrary.org/obo/GAZ_00068294">
        <rdf:type rdf:resource="http://purl.obolibrary.org/obo/ENVO_00000856"/>
        <obo:RO_0001025 rdf:resource="http://purl.obolibrary.org/obo/GAZ_00000541"/>
        <obo:IAO_0000115>A municipality in the Solola Department of Guatemala.</obo:IAO_0000115>
        <oboInOwl:hasOBONamespace>GAZ</oboInOwl:hasOBONamespace>
        <oboInOwl:id>GAZ:00068294</oboInOwl:id>
        <rdfs:label>Municipality of Santiago Atitlan</rdfs:label>
    </owl:NamedIndividual>
    


    <!-- http://purl.obolibrary.org/obo/GAZ_00068295 -->

    <owl:NamedIndividual rdf:about="http://purl.obolibrary.org/obo/GAZ_00068295">
        <rdf:type rdf:resource="http://purl.obolibrary.org/obo/ENVO_00000856"/>
        <obo:RO_0001025 rdf:resource="http://purl.obolibrary.org/obo/GAZ_00000541"/>
        <obo:IAO_0000115>A municipality in the Solola Department of Guatemala.</obo:IAO_0000115>
        <oboInOwl:hasOBONamespace>GAZ</oboInOwl:hasOBONamespace>
        <oboInOwl:id>GAZ:00068295</oboInOwl:id>
        <rdfs:label>Municipality of San Pablo La Laguna</rdfs:label>
    </owl:NamedIndividual>
    


    <!-- http://purl.obolibrary.org/obo/GAZ_00068296 -->

    <owl:NamedIndividual rdf:about="http://purl.obolibrary.org/obo/GAZ_00068296">
        <rdf:type rdf:resource="http://purl.obolibrary.org/obo/ENVO_00000856"/>
        <obo:RO_0001025 rdf:resource="http://purl.obolibrary.org/obo/GAZ_00000541"/>
        <obo:IAO_0000115>A municipality in the Solola Department of Guatemala.</obo:IAO_0000115>
        <oboInOwl:hasOBONamespace>GAZ</oboInOwl:hasOBONamespace>
        <oboInOwl:id>GAZ:00068296</oboInOwl:id>
        <rdfs:label>Municipality of Solola</rdfs:label>
    </owl:NamedIndividual>
    


    <!-- http://purl.obolibrary.org/obo/GAZ_00068297 -->

    <owl:NamedIndividual rdf:about="http://purl.obolibrary.org/obo/GAZ_00068297">
        <rdf:type rdf:resource="http://purl.obolibrary.org/obo/ENVO_00000856"/>
        <obo:RO_0001025 rdf:resource="http://purl.obolibrary.org/obo/GAZ_00000541"/>
        <obo:IAO_0000115>A municipality in the Solola Department of Guatemala.</obo:IAO_0000115>
        <oboInOwl:hasOBONamespace>GAZ</oboInOwl:hasOBONamespace>
        <oboInOwl:id>GAZ:00068297</oboInOwl:id>
        <rdfs:label>Municipality of San Juan La Laguna</rdfs:label>
    </owl:NamedIndividual>
    


    <!-- http://purl.obolibrary.org/obo/GAZ_00068298 -->

    <owl:NamedIndividual rdf:about="http://purl.obolibrary.org/obo/GAZ_00068298">
        <rdf:type rdf:resource="http://purl.obolibrary.org/obo/ENVO_00000856"/>
        <obo:RO_0001025 rdf:resource="http://purl.obolibrary.org/obo/GAZ_00000541"/>
        <obo:IAO_0000115>A municipality in the Solola Department of Guatemala.</obo:IAO_0000115>
        <oboInOwl:hasOBONamespace>GAZ</oboInOwl:hasOBONamespace>
        <oboInOwl:id>GAZ:00068298</oboInOwl:id>
        <rdfs:label>Municipality of Santa Catarina Palopo</rdfs:label>
    </owl:NamedIndividual>
    


    <!-- http://purl.obolibrary.org/obo/GAZ_00068299 -->

    <owl:NamedIndividual rdf:about="http://purl.obolibrary.org/obo/GAZ_00068299">
        <rdf:type rdf:resource="http://purl.obolibrary.org/obo/ENVO_00000856"/>
        <obo:RO_0001025 rdf:resource="http://purl.obolibrary.org/obo/GAZ_00000541"/>
        <obo:IAO_0000115>A municipality in the Solola Department of Guatemala.</obo:IAO_0000115>
        <oboInOwl:hasOBONamespace>GAZ</oboInOwl:hasOBONamespace>
        <oboInOwl:id>GAZ:00068299</oboInOwl:id>
        <rdfs:label>Municipality of San Jose Chacaya</rdfs:label>
    </owl:NamedIndividual>
    


    <!-- http://purl.obolibrary.org/obo/GAZ_00068300 -->

    <owl:NamedIndividual rdf:about="http://purl.obolibrary.org/obo/GAZ_00068300">
        <rdf:type rdf:resource="http://purl.obolibrary.org/obo/ENVO_00000856"/>
        <obo:RO_0001025 rdf:resource="http://purl.obolibrary.org/obo/GAZ_00000541"/>
        <obo:IAO_0000115>A municipality in the Solola Department of Guatemala.</obo:IAO_0000115>
        <oboInOwl:hasOBONamespace>GAZ</oboInOwl:hasOBONamespace>
        <oboInOwl:id>GAZ:00068300</oboInOwl:id>
        <rdfs:label>Municipality of San Pedro La Laguna</rdfs:label>
    </owl:NamedIndividual>
    


    <!-- http://purl.obolibrary.org/obo/GAZ_00068303 -->

    <owl:NamedIndividual rdf:about="http://purl.obolibrary.org/obo/GAZ_00068303">
        <rdf:type rdf:resource="http://purl.obolibrary.org/obo/ENVO_00000856"/>
        <obo:RO_0001025 rdf:resource="http://purl.obolibrary.org/obo/GAZ_00000541"/>
        <obo:IAO_0000115>A municipality in the Solola Department of Guatemala.</obo:IAO_0000115>
        <oboInOwl:hasOBONamespace>GAZ</oboInOwl:hasOBONamespace>
        <oboInOwl:id>GAZ:00068303</oboInOwl:id>
        <rdfs:label>Municipality of San Lucas Toliman</rdfs:label>
    </owl:NamedIndividual>
    


    <!-- http://purl.obolibrary.org/obo/GAZ_00068304 -->

    <owl:NamedIndividual rdf:about="http://purl.obolibrary.org/obo/GAZ_00068304">
        <rdf:type rdf:resource="http://purl.obolibrary.org/obo/ENVO_00000856"/>
        <obo:RO_0001025 rdf:resource="http://purl.obolibrary.org/obo/GAZ_00000545"/>
        <obo:IAO_0000115>A municipality in the Suchitepequez Department of Guatemala.</obo:IAO_0000115>
        <oboInOwl:hasOBONamespace>GAZ</oboInOwl:hasOBONamespace>
        <oboInOwl:id>GAZ:00068304</oboInOwl:id>
        <rdfs:label>Municipality of Rio Bravo</rdfs:label>
    </owl:NamedIndividual>
    


    <!-- http://purl.obolibrary.org/obo/GAZ_00068305 -->

    <owl:NamedIndividual rdf:about="http://purl.obolibrary.org/obo/GAZ_00068305">
        <rdf:type rdf:resource="http://purl.obolibrary.org/obo/ENVO_00000856"/>
        <obo:RO_0001025 rdf:resource="http://purl.obolibrary.org/obo/GAZ_00000545"/>
        <obo:IAO_0000115>A municipality in the Suchitepequez Department of Guatemala.</obo:IAO_0000115>
        <oboInOwl:hasOBONamespace>GAZ</oboInOwl:hasOBONamespace>
        <oboInOwl:id>GAZ:00068305</oboInOwl:id>
        <rdfs:label>Municipality of Patulul</rdfs:label>
    </owl:NamedIndividual>
    


    <!-- http://purl.obolibrary.org/obo/GAZ_00068306 -->

    <owl:NamedIndividual rdf:about="http://purl.obolibrary.org/obo/GAZ_00068306">
        <rdf:type rdf:resource="http://purl.obolibrary.org/obo/ENVO_00000856"/>
        <obo:RO_0001025 rdf:resource="http://purl.obolibrary.org/obo/GAZ_00000541"/>
        <obo:IAO_0000115>A municipality in the Solola Department of Guatemala.</obo:IAO_0000115>
        <oboInOwl:hasOBONamespace>GAZ</oboInOwl:hasOBONamespace>
        <oboInOwl:id>GAZ:00068306</oboInOwl:id>
        <rdfs:label>Municipality of San Marcos La Laguna</rdfs:label>
    </owl:NamedIndividual>
    


    <!-- http://purl.obolibrary.org/obo/GAZ_00068307 -->

    <owl:NamedIndividual rdf:about="http://purl.obolibrary.org/obo/GAZ_00068307">
        <rdf:type rdf:resource="http://purl.obolibrary.org/obo/ENVO_00000856"/>
        <obo:RO_0001025 rdf:resource="http://purl.obolibrary.org/obo/GAZ_00000545"/>
        <obo:IAO_0000115>A municipality in the Suchitepequez Department of Guatemala.</obo:IAO_0000115>
        <oboInOwl:hasOBONamespace>GAZ</oboInOwl:hasOBONamespace>
        <oboInOwl:id>GAZ:00068307</oboInOwl:id>
        <rdfs:label>Municipality of Cuyotenango</rdfs:label>
    </owl:NamedIndividual>
    


    <!-- http://purl.obolibrary.org/obo/GAZ_00068308 -->

    <owl:NamedIndividual rdf:about="http://purl.obolibrary.org/obo/GAZ_00068308">
        <rdf:type rdf:resource="http://purl.obolibrary.org/obo/ENVO_00000856"/>
        <obo:RO_0001025 rdf:resource="http://purl.obolibrary.org/obo/GAZ_00000545"/>
        <obo:IAO_0000115>A municipality in the Suchitepequez Department of Guatemala.</obo:IAO_0000115>
        <oboInOwl:hasOBONamespace>GAZ</oboInOwl:hasOBONamespace>
        <oboInOwl:id>GAZ:00068308</oboInOwl:id>
        <rdfs:label>Municipality of Mazatenango</rdfs:label>
    </owl:NamedIndividual>
    


    <!-- http://purl.obolibrary.org/obo/GAZ_00068309 -->

    <owl:NamedIndividual rdf:about="http://purl.obolibrary.org/obo/GAZ_00068309">
        <rdf:type rdf:resource="http://purl.obolibrary.org/obo/ENVO_00000856"/>
        <obo:RO_0001025 rdf:resource="http://purl.obolibrary.org/obo/GAZ_00000545"/>
        <obo:IAO_0000115>A municipality in the Suchitepequez Department of Guatemala.</obo:IAO_0000115>
        <oboInOwl:hasOBONamespace>GAZ</oboInOwl:hasOBONamespace>
        <oboInOwl:id>GAZ:00068309</oboInOwl:id>
        <rdfs:label>Municipality of San Miguel Panan</rdfs:label>
    </owl:NamedIndividual>
    


    <!-- http://purl.obolibrary.org/obo/GAZ_00068310 -->

    <owl:NamedIndividual rdf:about="http://purl.obolibrary.org/obo/GAZ_00068310">
        <rdf:type rdf:resource="http://purl.obolibrary.org/obo/ENVO_00000856"/>
        <obo:RO_0001025 rdf:resource="http://purl.obolibrary.org/obo/GAZ_00000545"/>
        <obo:IAO_0000115>A municipality in the Suchitepequez Department of Guatemala.</obo:IAO_0000115>
        <oboInOwl:hasOBONamespace>GAZ</oboInOwl:hasOBONamespace>
        <oboInOwl:id>GAZ:00068310</oboInOwl:id>
        <rdfs:label>Municipality of San Jose El Idolo</rdfs:label>
    </owl:NamedIndividual>
    


    <!-- http://purl.obolibrary.org/obo/GAZ_00068311 -->

    <owl:NamedIndividual rdf:about="http://purl.obolibrary.org/obo/GAZ_00068311">
        <rdf:type rdf:resource="http://purl.obolibrary.org/obo/ENVO_00000856"/>
        <obo:RO_0001025 rdf:resource="http://purl.obolibrary.org/obo/GAZ_00000545"/>
        <obo:IAO_0000115>A municipality in the Suchitepequez Department of Guatemala.</obo:IAO_0000115>
        <oboInOwl:hasOBONamespace>GAZ</oboInOwl:hasOBONamespace>
        <oboInOwl:id>GAZ:00068311</oboInOwl:id>
        <rdfs:label>Municipality of San Gabriel</rdfs:label>
    </owl:NamedIndividual>
    


    <!-- http://purl.obolibrary.org/obo/GAZ_00068312 -->

    <owl:NamedIndividual rdf:about="http://purl.obolibrary.org/obo/GAZ_00068312">
        <rdf:type rdf:resource="http://purl.obolibrary.org/obo/ENVO_00000856"/>
        <obo:RO_0001025 rdf:resource="http://purl.obolibrary.org/obo/GAZ_00000545"/>
        <obo:IAO_0000115>A municipality in the Suchitepequez Department of Guatemala.</obo:IAO_0000115>
        <oboInOwl:hasOBONamespace>GAZ</oboInOwl:hasOBONamespace>
        <oboInOwl:id>GAZ:00068312</oboInOwl:id>
        <rdfs:label>Municipality of Santa Barbara</rdfs:label>
    </owl:NamedIndividual>
    


    <!-- http://purl.obolibrary.org/obo/GAZ_00068313 -->

    <owl:NamedIndividual rdf:about="http://purl.obolibrary.org/obo/GAZ_00068313">
        <rdf:type rdf:resource="http://purl.obolibrary.org/obo/ENVO_00000856"/>
        <obo:RO_0001025 rdf:resource="http://purl.obolibrary.org/obo/GAZ_00000545"/>
        <obo:IAO_0000115>A municipality in the Suchitepequez Department of Guatemala.</obo:IAO_0000115>
        <oboInOwl:hasOBONamespace>GAZ</oboInOwl:hasOBONamespace>
        <oboInOwl:id>GAZ:00068313</oboInOwl:id>
        <rdfs:label>Municipality of Santo Tomas La Union</rdfs:label>
    </owl:NamedIndividual>
    


    <!-- http://purl.obolibrary.org/obo/GAZ_00068314 -->

    <owl:NamedIndividual rdf:about="http://purl.obolibrary.org/obo/GAZ_00068314">
        <rdf:type rdf:resource="http://purl.obolibrary.org/obo/ENVO_00000856"/>
        <obo:RO_0001025 rdf:resource="http://purl.obolibrary.org/obo/GAZ_00000545"/>
        <obo:IAO_0000115>A municipality in the Suchitepequez Department of Guatemala.</obo:IAO_0000115>
        <oboInOwl:hasOBONamespace>GAZ</oboInOwl:hasOBONamespace>
        <oboInOwl:id>GAZ:00068314</oboInOwl:id>
        <rdfs:label>Municipality of Pueblo Nuevo</rdfs:label>
    </owl:NamedIndividual>
    


    <!-- http://purl.obolibrary.org/obo/GAZ_00068315 -->

    <owl:NamedIndividual rdf:about="http://purl.obolibrary.org/obo/GAZ_00068315">
        <rdf:type rdf:resource="http://purl.obolibrary.org/obo/ENVO_00000856"/>
        <obo:RO_0001025 rdf:resource="http://purl.obolibrary.org/obo/GAZ_00000545"/>
        <obo:IAO_0000115>A municipality in the Suchitepequez Department of Guatemala.</obo:IAO_0000115>
        <oboInOwl:hasOBONamespace>GAZ</oboInOwl:hasOBONamespace>
        <oboInOwl:id>GAZ:00068315</oboInOwl:id>
        <rdfs:label>Municipality of San Lorenzo</rdfs:label>
    </owl:NamedIndividual>
    


    <!-- http://purl.obolibrary.org/obo/GAZ_00068316 -->

    <owl:NamedIndividual rdf:about="http://purl.obolibrary.org/obo/GAZ_00068316">
        <rdf:type rdf:resource="http://purl.obolibrary.org/obo/ENVO_00000856"/>
        <obo:RO_0001025 rdf:resource="http://purl.obolibrary.org/obo/GAZ_00000545"/>
        <obo:IAO_0000115>A municipality in the Suchitepequez Department of Guatemala.</obo:IAO_0000115>
        <oboInOwl:hasOBONamespace>GAZ</oboInOwl:hasOBONamespace>
        <oboInOwl:id>GAZ:00068316</oboInOwl:id>
        <rdfs:label>Municipality of San Pablo Jocopilas</rdfs:label>
    </owl:NamedIndividual>
    


    <!-- http://purl.obolibrary.org/obo/GAZ_00068317 -->

    <owl:NamedIndividual rdf:about="http://purl.obolibrary.org/obo/GAZ_00068317">
        <rdf:type rdf:resource="http://purl.obolibrary.org/obo/ENVO_00000856"/>
        <obo:RO_0001025 rdf:resource="http://purl.obolibrary.org/obo/GAZ_00000545"/>
        <obo:IAO_0000115>A municipality in the Suchitepequez Department of Guatemala.</obo:IAO_0000115>
        <oboInOwl:hasOBONamespace>GAZ</oboInOwl:hasOBONamespace>
        <oboInOwl:id>GAZ:00068317</oboInOwl:id>
        <rdfs:label>Municipality of Zunilito</rdfs:label>
    </owl:NamedIndividual>
    


    <!-- http://purl.obolibrary.org/obo/GAZ_00068318 -->

    <owl:NamedIndividual rdf:about="http://purl.obolibrary.org/obo/GAZ_00068318">
        <rdf:type rdf:resource="http://purl.obolibrary.org/obo/ENVO_00000856"/>
        <obo:RO_0001025 rdf:resource="http://purl.obolibrary.org/obo/GAZ_00000545"/>
        <obo:IAO_0000115>A municipality in the Suchitepequez Department of Guatemala.</obo:IAO_0000115>
        <oboInOwl:hasOBONamespace>GAZ</oboInOwl:hasOBONamespace>
        <oboInOwl:id>GAZ:00068318</oboInOwl:id>
        <rdfs:label>Municipality of San Bernardino</rdfs:label>
    </owl:NamedIndividual>
    


    <!-- http://purl.obolibrary.org/obo/GAZ_00068319 -->

    <owl:NamedIndividual rdf:about="http://purl.obolibrary.org/obo/GAZ_00068319">
        <rdf:type rdf:resource="http://purl.obolibrary.org/obo/ENVO_00000856"/>
        <obo:RO_0001025 rdf:resource="http://purl.obolibrary.org/obo/GAZ_00000545"/>
        <obo:IAO_0000115>A municipality in the Suchitepequez Department of Guatemala.</obo:IAO_0000115>
        <oboInOwl:hasOBONamespace>GAZ</oboInOwl:hasOBONamespace>
        <oboInOwl:id>GAZ:00068319</oboInOwl:id>
        <rdfs:label>Municipality of Santo Domingo Suchitepequez</rdfs:label>
    </owl:NamedIndividual>
    


    <!-- http://purl.obolibrary.org/obo/GAZ_00068320 -->

    <owl:NamedIndividual rdf:about="http://purl.obolibrary.org/obo/GAZ_00068320">
        <rdf:type rdf:resource="http://purl.obolibrary.org/obo/ENVO_00000856"/>
        <obo:RO_0001025 rdf:resource="http://purl.obolibrary.org/obo/GAZ_00000545"/>
        <obo:IAO_0000115>A municipality in the Suchitepequez Department of Guatemala.</obo:IAO_0000115>
        <oboInOwl:hasOBONamespace>GAZ</oboInOwl:hasOBONamespace>
        <oboInOwl:id>GAZ:00068320</oboInOwl:id>
        <rdfs:label>Municipality of San Juan Bautista</rdfs:label>
    </owl:NamedIndividual>
    


    <!-- http://purl.obolibrary.org/obo/GAZ_00068321 -->

    <owl:NamedIndividual rdf:about="http://purl.obolibrary.org/obo/GAZ_00068321">
        <rdf:type rdf:resource="http://purl.obolibrary.org/obo/ENVO_00000856"/>
        <obo:RO_0001025 rdf:resource="http://purl.obolibrary.org/obo/GAZ_00000545"/>
        <obo:IAO_0000115>A municipality in the Suchitepequez Department of Guatemala.</obo:IAO_0000115>
        <oboInOwl:hasOBONamespace>GAZ</oboInOwl:hasOBONamespace>
        <oboInOwl:id>GAZ:00068321</oboInOwl:id>
        <rdfs:label>Municipality of San Francisco Zapotitlan</rdfs:label>
    </owl:NamedIndividual>
    


    <!-- http://purl.obolibrary.org/obo/GAZ_00068322 -->

    <owl:NamedIndividual rdf:about="http://purl.obolibrary.org/obo/GAZ_00068322">
        <rdf:type rdf:resource="http://purl.obolibrary.org/obo/ENVO_00000856"/>
        <obo:RO_0001025 rdf:resource="http://purl.obolibrary.org/obo/GAZ_00000545"/>
        <obo:IAO_0000115>A municipality in the Suchitepequez Department of Guatemala.</obo:IAO_0000115>
        <oboInOwl:hasOBONamespace>GAZ</oboInOwl:hasOBONamespace>
        <oboInOwl:id>GAZ:00068322</oboInOwl:id>
        <rdfs:label>Municipality of Samayac</rdfs:label>
    </owl:NamedIndividual>
    


    <!-- http://purl.obolibrary.org/obo/GAZ_00068323 -->

    <owl:NamedIndividual rdf:about="http://purl.obolibrary.org/obo/GAZ_00068323">
        <rdf:type rdf:resource="http://purl.obolibrary.org/obo/ENVO_00000856"/>
        <obo:RO_0001025 rdf:resource="http://purl.obolibrary.org/obo/GAZ_00000545"/>
        <obo:IAO_0000115>A municipality in the Suchitepequez Department of Guatemala.</obo:IAO_0000115>
        <oboInOwl:hasOBONamespace>GAZ</oboInOwl:hasOBONamespace>
        <oboInOwl:id>GAZ:00068323</oboInOwl:id>
        <rdfs:label>Municipality of Chicacao</rdfs:label>
    </owl:NamedIndividual>
    


    <!-- http://purl.obolibrary.org/obo/GAZ_00068324 -->

    <owl:NamedIndividual rdf:about="http://purl.obolibrary.org/obo/GAZ_00068324">
        <rdf:type rdf:resource="http://purl.obolibrary.org/obo/ENVO_00000856"/>
        <obo:RO_0001025 rdf:resource="http://purl.obolibrary.org/obo/GAZ_00000549"/>
        <obo:IAO_0000115>A municipality in the Totonicapan Department of Guatemala.</obo:IAO_0000115>
        <oboInOwl:hasOBONamespace>GAZ</oboInOwl:hasOBONamespace>
        <oboInOwl:id>GAZ:00068324</oboInOwl:id>
        <rdfs:label>Municipality of Momostenango</rdfs:label>
    </owl:NamedIndividual>
    


    <!-- http://purl.obolibrary.org/obo/GAZ_00068325 -->

    <owl:NamedIndividual rdf:about="http://purl.obolibrary.org/obo/GAZ_00068325">
        <rdf:type rdf:resource="http://purl.obolibrary.org/obo/ENVO_00000856"/>
        <obo:RO_0001025 rdf:resource="http://purl.obolibrary.org/obo/GAZ_00000549"/>
        <obo:IAO_0000115>A municipality in the Totonicapan Department of Guatemala.</obo:IAO_0000115>
        <oboInOwl:hasOBONamespace>GAZ</oboInOwl:hasOBONamespace>
        <oboInOwl:id>GAZ:00068325</oboInOwl:id>
        <rdfs:label>Municipality of San Bartolo</rdfs:label>
    </owl:NamedIndividual>
    


    <!-- http://purl.obolibrary.org/obo/GAZ_00068326 -->

    <owl:NamedIndividual rdf:about="http://purl.obolibrary.org/obo/GAZ_00068326">
        <rdf:type rdf:resource="http://purl.obolibrary.org/obo/ENVO_00000856"/>
        <obo:RO_0001025 rdf:resource="http://purl.obolibrary.org/obo/GAZ_00000549"/>
        <obo:IAO_0000115>A municipality in the Totonicapan Department of Guatemala.</obo:IAO_0000115>
        <oboInOwl:hasOBONamespace>GAZ</oboInOwl:hasOBONamespace>
        <oboInOwl:id>GAZ:00068326</oboInOwl:id>
        <rdfs:label>Municipality of San Andres Xecul</rdfs:label>
    </owl:NamedIndividual>
    


    <!-- http://purl.obolibrary.org/obo/GAZ_00068327 -->

    <owl:NamedIndividual rdf:about="http://purl.obolibrary.org/obo/GAZ_00068327">
        <rdf:type rdf:resource="http://purl.obolibrary.org/obo/ENVO_00000856"/>
        <obo:RO_0001025 rdf:resource="http://purl.obolibrary.org/obo/GAZ_00000549"/>
        <obo:IAO_0000115>A municipality in the Totonicapan Department of Guatemala.</obo:IAO_0000115>
        <oboInOwl:hasOBONamespace>GAZ</oboInOwl:hasOBONamespace>
        <oboInOwl:id>GAZ:00068327</oboInOwl:id>
        <rdfs:label>Municipality of San Cristobal Totonicapan</rdfs:label>
    </owl:NamedIndividual>
    


    <!-- http://purl.obolibrary.org/obo/GAZ_00068328 -->

    <owl:NamedIndividual rdf:about="http://purl.obolibrary.org/obo/GAZ_00068328">
        <rdf:type rdf:resource="http://purl.obolibrary.org/obo/ENVO_00000856"/>
        <obo:RO_0001025 rdf:resource="http://purl.obolibrary.org/obo/GAZ_00000549"/>
        <obo:IAO_0000115>A municipality in the Totonicapan Department of Guatemala.</obo:IAO_0000115>
        <oboInOwl:hasOBONamespace>GAZ</oboInOwl:hasOBONamespace>
        <oboInOwl:id>GAZ:00068328</oboInOwl:id>
        <rdfs:label>Municipality of Santa Maria Chiquimula</rdfs:label>
    </owl:NamedIndividual>
    


    <!-- http://purl.obolibrary.org/obo/GAZ_00068329 -->

    <owl:NamedIndividual rdf:about="http://purl.obolibrary.org/obo/GAZ_00068329">
        <rdf:type rdf:resource="http://purl.obolibrary.org/obo/ENVO_00000856"/>
        <obo:RO_0001025 rdf:resource="http://purl.obolibrary.org/obo/GAZ_00000549"/>
        <obo:IAO_0000115>A municipality in the Totonicapan Department of Guatemala.</obo:IAO_0000115>
        <oboInOwl:hasOBONamespace>GAZ</oboInOwl:hasOBONamespace>
        <oboInOwl:id>GAZ:00068329</oboInOwl:id>
        <rdfs:label>Municipality of Totonicapan</rdfs:label>
    </owl:NamedIndividual>
    


    <!-- http://purl.obolibrary.org/obo/GAZ_00068330 -->

    <owl:NamedIndividual rdf:about="http://purl.obolibrary.org/obo/GAZ_00068330">
        <rdf:type rdf:resource="http://purl.obolibrary.org/obo/ENVO_00000856"/>
        <obo:RO_0001025 rdf:resource="http://purl.obolibrary.org/obo/GAZ_00000549"/>
        <obo:IAO_0000115>A municipality in the Totonicapan Department of Guatemala.</obo:IAO_0000115>
        <oboInOwl:hasOBONamespace>GAZ</oboInOwl:hasOBONamespace>
        <oboInOwl:id>GAZ:00068330</oboInOwl:id>
        <rdfs:label>Municipality of Santa Lucia La Reforma</rdfs:label>
    </owl:NamedIndividual>
    


    <!-- http://purl.obolibrary.org/obo/GAZ_00068331 -->

    <owl:NamedIndividual rdf:about="http://purl.obolibrary.org/obo/GAZ_00068331">
        <rdf:type rdf:resource="http://purl.obolibrary.org/obo/ENVO_00000856"/>
        <obo:RO_0001025 rdf:resource="http://purl.obolibrary.org/obo/GAZ_00000549"/>
        <obo:IAO_0000115>A municipality in the Totonicapan Department of Guatemala.</obo:IAO_0000115>
        <oboInOwl:hasOBONamespace>GAZ</oboInOwl:hasOBONamespace>
        <oboInOwl:id>GAZ:00068331</oboInOwl:id>
        <rdfs:label>Municipality of San Francisco El Alto</rdfs:label>
    </owl:NamedIndividual>
    


    <!-- http://purl.obolibrary.org/obo/GAZ_00068332 -->

    <owl:NamedIndividual rdf:about="http://purl.obolibrary.org/obo/GAZ_00068332">
        <rdf:type rdf:resource="http://purl.obolibrary.org/obo/ENVO_00000856"/>
        <obo:RO_0001025 rdf:resource="http://purl.obolibrary.org/obo/GAZ_00000548"/>
        <obo:IAO_0000115>A municipality in the Guatemalan Department of Zacapa.</obo:IAO_0000115>
        <oboInOwl:hasOBONamespace>GAZ</oboInOwl:hasOBONamespace>
        <oboInOwl:id>GAZ:00068332</oboInOwl:id>
        <rdfs:label>Municipality of Estanzuela</rdfs:label>
    </owl:NamedIndividual>
    


    <!-- http://purl.obolibrary.org/obo/GAZ_00068333 -->

    <owl:NamedIndividual rdf:about="http://purl.obolibrary.org/obo/GAZ_00068333">
        <rdf:type rdf:resource="http://purl.obolibrary.org/obo/ENVO_00000856"/>
        <obo:RO_0001025 rdf:resource="http://purl.obolibrary.org/obo/GAZ_00000548"/>
        <obo:IAO_0000115>A municipality in the Guatemalan Department of Zacapa.</obo:IAO_0000115>
        <oboInOwl:hasOBONamespace>GAZ</oboInOwl:hasOBONamespace>
        <oboInOwl:id>GAZ:00068333</oboInOwl:id>
        <rdfs:label>Municipality of Gualan</rdfs:label>
    </owl:NamedIndividual>
    


    <!-- http://purl.obolibrary.org/obo/GAZ_00068334 -->

    <owl:NamedIndividual rdf:about="http://purl.obolibrary.org/obo/GAZ_00068334">
        <rdf:type rdf:resource="http://purl.obolibrary.org/obo/ENVO_00000856"/>
        <obo:RO_0001025 rdf:resource="http://purl.obolibrary.org/obo/GAZ_00000548"/>
        <obo:IAO_0000115>A municipality in the Guatemalan Department of Zacapa.</obo:IAO_0000115>
        <oboInOwl:hasOBONamespace>GAZ</oboInOwl:hasOBONamespace>
        <oboInOwl:id>GAZ:00068334</oboInOwl:id>
        <rdfs:label>Municipality of Cabanas</rdfs:label>
    </owl:NamedIndividual>
    


    <!-- http://purl.obolibrary.org/obo/GAZ_00068335 -->

    <owl:NamedIndividual rdf:about="http://purl.obolibrary.org/obo/GAZ_00068335">
        <rdf:type rdf:resource="http://purl.obolibrary.org/obo/ENVO_00000856"/>
        <obo:RO_0001025 rdf:resource="http://purl.obolibrary.org/obo/GAZ_00000548"/>
        <obo:IAO_0000115>A municipality in the Guatemalan Department of Zacapa.</obo:IAO_0000115>
        <oboInOwl:hasOBONamespace>GAZ</oboInOwl:hasOBONamespace>
        <oboInOwl:id>GAZ:00068335</oboInOwl:id>
        <rdfs:label>Municipality of Zacapa</rdfs:label>
    </owl:NamedIndividual>
    


    <!-- http://purl.obolibrary.org/obo/GAZ_00068336 -->

    <owl:NamedIndividual rdf:about="http://purl.obolibrary.org/obo/GAZ_00068336">
        <rdf:type rdf:resource="http://purl.obolibrary.org/obo/ENVO_00000856"/>
        <obo:RO_0001025 rdf:resource="http://purl.obolibrary.org/obo/GAZ_00000548"/>
        <obo:IAO_0000115>A municipality in the Guatemalan Department of Zacapa.</obo:IAO_0000115>
        <oboInOwl:hasOBONamespace>GAZ</oboInOwl:hasOBONamespace>
        <oboInOwl:id>GAZ:00068336</oboInOwl:id>
        <rdfs:label>Municipality of Huite</rdfs:label>
    </owl:NamedIndividual>
    


    <!-- http://purl.obolibrary.org/obo/GAZ_00068337 -->

    <owl:NamedIndividual rdf:about="http://purl.obolibrary.org/obo/GAZ_00068337">
        <rdf:type rdf:resource="http://purl.obolibrary.org/obo/ENVO_00000856"/>
        <obo:RO_0001025 rdf:resource="http://purl.obolibrary.org/obo/GAZ_00000548"/>
        <obo:IAO_0000115>A municipality in the Guatemalan Department of Zacapa.</obo:IAO_0000115>
        <oboInOwl:hasOBONamespace>GAZ</oboInOwl:hasOBONamespace>
        <oboInOwl:id>GAZ:00068337</oboInOwl:id>
        <rdfs:label>Municipality of San Diego</rdfs:label>
    </owl:NamedIndividual>
    


    <!-- http://purl.obolibrary.org/obo/GAZ_00068338 -->

    <owl:NamedIndividual rdf:about="http://purl.obolibrary.org/obo/GAZ_00068338">
        <rdf:type rdf:resource="http://purl.obolibrary.org/obo/ENVO_00000856"/>
        <obo:RO_0001025 rdf:resource="http://purl.obolibrary.org/obo/GAZ_00000548"/>
        <obo:IAO_0000115>A municipality in the Guatemalan Department of Zacapa.</obo:IAO_0000115>
        <oboInOwl:hasOBONamespace>GAZ</oboInOwl:hasOBONamespace>
        <oboInOwl:id>GAZ:00068338</oboInOwl:id>
        <rdfs:label>Municipality of Rio Hondo</rdfs:label>
    </owl:NamedIndividual>
    


    <!-- http://purl.obolibrary.org/obo/GAZ_00068339 -->

    <owl:NamedIndividual rdf:about="http://purl.obolibrary.org/obo/GAZ_00068339">
        <rdf:type rdf:resource="http://purl.obolibrary.org/obo/ENVO_00000856"/>
        <obo:RO_0001025 rdf:resource="http://purl.obolibrary.org/obo/GAZ_00000548"/>
        <obo:IAO_0000115>A municipality in the Guatemalan Department of Zacapa.</obo:IAO_0000115>
        <oboInOwl:hasOBONamespace>GAZ</oboInOwl:hasOBONamespace>
        <oboInOwl:id>GAZ:00068339</oboInOwl:id>
        <rdfs:label>Municipality of La Union</rdfs:label>
    </owl:NamedIndividual>
    


    <!-- http://purl.obolibrary.org/obo/GAZ_00068340 -->

    <owl:NamedIndividual rdf:about="http://purl.obolibrary.org/obo/GAZ_00068340">
        <obo:RO_0001025 rdf:resource="http://purl.obolibrary.org/obo/GAZ_00000433"/>
        <obo:IAO_0000115>A protected area.</obo:IAO_0000115>
        <oboInOwl:hasOBONamespace>GAZ</oboInOwl:hasOBONamespace>
        <oboInOwl:id>GAZ:00068340</oboInOwl:id>
        <rdfs:label>Mario Dary Biotope Preserve</rdfs:label>
    </owl:NamedIndividual>
    


    <!-- http://purl.obolibrary.org/obo/GAZ_00068341 -->

    <owl:NamedIndividual rdf:about="http://purl.obolibrary.org/obo/GAZ_00068341">
        <rdf:type rdf:resource="http://purl.obolibrary.org/obo/ENVO_00000856"/>
        <obo:RO_0001025 rdf:resource="http://purl.obolibrary.org/obo/GAZ_00000548"/>
        <obo:IAO_0000115>A municipality in the Guatemalan Department of Zacapa.</obo:IAO_0000115>
        <oboInOwl:hasOBONamespace>GAZ</oboInOwl:hasOBONamespace>
        <oboInOwl:id>GAZ:00068341</oboInOwl:id>
        <rdfs:label>Municipality of Usumatlan</rdfs:label>
    </owl:NamedIndividual>
    


    <!-- http://purl.obolibrary.org/obo/GAZ_00068342 -->

    <owl:NamedIndividual rdf:about="http://purl.obolibrary.org/obo/GAZ_00068342">
        <rdf:type rdf:resource="http://purl.obolibrary.org/obo/ENVO_00000856"/>
        <obo:RO_0001025 rdf:resource="http://purl.obolibrary.org/obo/GAZ_00000548"/>
        <obo:IAO_0000115>A municipality in the Guatemalan Department of Zacapa.</obo:IAO_0000115>
        <oboInOwl:hasOBONamespace>GAZ</oboInOwl:hasOBONamespace>
        <oboInOwl:id>GAZ:00068342</oboInOwl:id>
        <rdfs:label>Municipality of Teculutan</rdfs:label>
    </owl:NamedIndividual>
    


    <!-- http://purl.obolibrary.org/obo/GAZ_00146412 -->

    <owl:NamedIndividual rdf:about="http://purl.obolibrary.org/obo/GAZ_00146412">
        <obo:IAO_0000115>A large bay in Central America. It is a part of Gulf of Honduras. Most of the bay is a part of Guatemala, while the western portion is a part of Belize.</obo:IAO_0000115>
        <oboInOwl:hasOBONamespace>GAZ</oboInOwl:hasOBONamespace>
        <oboInOwl:id>GAZ:00146412</oboInOwl:id>
        <rdfs:label>Bahia de Amatique</rdfs:label>
    </owl:NamedIndividual>
    


    <!-- http://purl.obolibrary.org/obo/GAZ_00248417 -->

    <owl:NamedIndividual rdf:about="http://purl.obolibrary.org/obo/GAZ_00248417">
        <obo:RO_0001025 rdf:resource="http://purl.obolibrary.org/obo/GAZ_00000529"/>
        <obo:IAO_0000115>Brackish lagoons on the Pacific Coast. Located 40 km W of Mazatenango.</obo:IAO_0000115>
        <oboInOwl:hasOBONamespace>GAZ</oboInOwl:hasOBONamespace>
        <oboInOwl:id>GAZ:00248417</oboInOwl:id>
        <rdfs:label>Manchon Lagoons</rdfs:label>
    </owl:NamedIndividual>
    


    <!-- http://purl.obolibrary.org/obo/GAZ_00248450 -->

    <owl:NamedIndividual rdf:about="http://purl.obolibrary.org/obo/GAZ_00248450">
        <obo:RO_0001025 rdf:resource="http://purl.obolibrary.org/obo/GAZ_00000477"/>
        <obo:IAO_0000115>A river.</obo:IAO_0000115>
        <oboInOwl:hasOBONamespace>GAZ</oboInOwl:hasOBONamespace>
        <oboInOwl:id>GAZ:00248450</oboInOwl:id>
        <rdfs:label>Rio Acome</rdfs:label>
    </owl:NamedIndividual>
    


    <!-- http://purl.obolibrary.org/obo/GAZ_00248527 -->

    <owl:NamedIndividual rdf:about="http://purl.obolibrary.org/obo/GAZ_00248527">
        <obo:RO_0001025 rdf:resource="http://purl.obolibrary.org/obo/GAZ_00248450"/>
        <obo:IAO_0000115>The estuary of the Rio Acome.</obo:IAO_0000115>
        <oboInOwl:hasOBONamespace>GAZ</oboInOwl:hasOBONamespace>
        <oboInOwl:id>GAZ:00248527</oboInOwl:id>
        <rdfs:label>Rio Acome Estuary</rdfs:label>
    </owl:NamedIndividual>
    


    <!-- http://purl.obolibrary.org/obo/GAZ_00248528 -->

    <owl:NamedIndividual rdf:about="http://purl.obolibrary.org/obo/GAZ_00248528">
        <obo:RO_0001025 rdf:resource="http://purl.obolibrary.org/obo/GAZ_00000540"/>
        <obo:IAO_0000115>Coastal brackish lagoons. Located 15 km S of Taxisco.</obo:IAO_0000115>
        <oboInOwl:hasOBONamespace>GAZ</oboInOwl:hasOBONamespace>
        <oboInOwl:id>GAZ:00248528</oboInOwl:id>
        <rdfs:label>Monterrico Lagoons</rdfs:label>
    </owl:NamedIndividual>
    


    <!-- http://purl.obolibrary.org/obo/GAZ_00248530 -->

    <owl:NamedIndividual rdf:about="http://purl.obolibrary.org/obo/GAZ_00248530">
        <obo:IAO_0000115>The estuary of the Rio Paz. Located 30 km SE of Taxisco.</obo:IAO_0000115>
        <oboInOwl:hasOBONamespace>GAZ</oboInOwl:hasOBONamespace>
        <oboInOwl:id>GAZ:00248530</oboInOwl:id>
        <rdfs:label>Rio Paz Estuary</rdfs:label>
    </owl:NamedIndividual>
    


    <!-- http://purl.obolibrary.org/obo/GAZ_00248531 -->

    <owl:NamedIndividual rdf:about="http://purl.obolibrary.org/obo/GAZ_00248531">
        <obo:RO_0001025 rdf:resource="http://purl.obolibrary.org/obo/GAZ_00000499"/>
        <obo:IAO_0000115>A freshwater lake. Located 37 km ESE of Taxisco.</obo:IAO_0000115>
        <oboInOwl:hasOBONamespace>GAZ</oboInOwl:hasOBONamespace>
        <oboInOwl:id>GAZ:00248531</oboInOwl:id>
        <rdfs:label>Laguna Grande</rdfs:label>
    </owl:NamedIndividual>
    


    <!-- http://purl.obolibrary.org/obo/GAZ_00248533 -->

    <owl:NamedIndividual rdf:about="http://purl.obolibrary.org/obo/GAZ_00248533">
        <obo:RO_0001025 rdf:resource="http://purl.obolibrary.org/obo/GAZ_00000540"/>
        <obo:IAO_0000115>A brackish lake of volcanic origin. Located 45 km ESE of Guatemala City.</obo:IAO_0000115>
        <oboInOwl:hasOBONamespace>GAZ</oboInOwl:hasOBONamespace>
        <oboInOwl:id>GAZ:00248533</oboInOwl:id>
        <rdfs:label>Laguna de Ayarza</rdfs:label>
    </owl:NamedIndividual>
    


    <!-- http://purl.obolibrary.org/obo/GAZ_00248534 -->

    <owl:NamedIndividual rdf:about="http://purl.obolibrary.org/obo/GAZ_00248534">
        <obo:RO_0001025 rdf:resource="http://purl.obolibrary.org/obo/GAZ_00266174"/>
        <obo:IAO_0000115>An almost freshwater lake. Located 30 km ESE of Guatamala City.</obo:IAO_0000115>
        <oboInOwl:hasOBONamespace>GAZ</oboInOwl:hasOBONamespace>
        <oboInOwl:id>GAZ:00248534</oboInOwl:id>
        <rdfs:label>Laguna El Pino</rdfs:label>
    </owl:NamedIndividual>
    


    <!-- http://purl.obolibrary.org/obo/GAZ_00248535 -->

    <owl:NamedIndividual rdf:about="http://purl.obolibrary.org/obo/GAZ_00248535">
        <obo:RO_0001025 rdf:resource="http://purl.obolibrary.org/obo/GAZ_00005154"/>
        <obo:IAO_0000115>One of the 22 administrative divisions of Guatamala City.</obo:IAO_0000115>
        <oboInOwl:hasOBONamespace>GAZ</oboInOwl:hasOBONamespace>
        <oboInOwl:id>GAZ:00248535</oboInOwl:id>
        <rdfs:label>Zone 1</rdfs:label>
    </owl:NamedIndividual>
    


    <!-- http://purl.obolibrary.org/obo/GAZ_00248536 -->

    <owl:NamedIndividual rdf:about="http://purl.obolibrary.org/obo/GAZ_00248536">
        <obo:RO_0001025 rdf:resource="http://purl.obolibrary.org/obo/GAZ_00005154"/>
        <obo:IAO_0000115>One of the 22 administrative divisions of Guatamala City.</obo:IAO_0000115>
        <oboInOwl:hasOBONamespace>GAZ</oboInOwl:hasOBONamespace>
        <oboInOwl:id>GAZ:00248536</oboInOwl:id>
        <rdfs:label>Zone 2</rdfs:label>
    </owl:NamedIndividual>
    


    <!-- http://purl.obolibrary.org/obo/GAZ_00248537 -->

    <owl:NamedIndividual rdf:about="http://purl.obolibrary.org/obo/GAZ_00248537">
        <obo:RO_0001025 rdf:resource="http://purl.obolibrary.org/obo/GAZ_00005154"/>
        <obo:IAO_0000115>One of the 22 administrative divisions of Guatamala City.</obo:IAO_0000115>
        <oboInOwl:hasOBONamespace>GAZ</oboInOwl:hasOBONamespace>
        <oboInOwl:id>GAZ:00248537</oboInOwl:id>
        <rdfs:label>Zone 3</rdfs:label>
    </owl:NamedIndividual>
    


    <!-- http://purl.obolibrary.org/obo/GAZ_00248538 -->

    <owl:NamedIndividual rdf:about="http://purl.obolibrary.org/obo/GAZ_00248538">
        <obo:RO_0001025 rdf:resource="http://purl.obolibrary.org/obo/GAZ_00005154"/>
        <obo:IAO_0000115>One of the 22 administrative divisions of Guatamala City.</obo:IAO_0000115>
        <oboInOwl:hasOBONamespace>GAZ</oboInOwl:hasOBONamespace>
        <oboInOwl:id>GAZ:00248538</oboInOwl:id>
        <rdfs:label>Zone 4</rdfs:label>
    </owl:NamedIndividual>
    


    <!-- http://purl.obolibrary.org/obo/GAZ_00248539 -->

    <owl:NamedIndividual rdf:about="http://purl.obolibrary.org/obo/GAZ_00248539">
        <obo:RO_0001025 rdf:resource="http://purl.obolibrary.org/obo/GAZ_00005154"/>
        <obo:IAO_0000115>One of the 22 administrative divisions of Guatamala City.</obo:IAO_0000115>
        <oboInOwl:hasOBONamespace>GAZ</oboInOwl:hasOBONamespace>
        <oboInOwl:id>GAZ:00248539</oboInOwl:id>
        <rdfs:label>Zone 5</rdfs:label>
    </owl:NamedIndividual>
    


    <!-- http://purl.obolibrary.org/obo/GAZ_00248540 -->

    <owl:NamedIndividual rdf:about="http://purl.obolibrary.org/obo/GAZ_00248540">
        <obo:RO_0001025 rdf:resource="http://purl.obolibrary.org/obo/GAZ_00005154"/>
        <obo:IAO_0000115>One of the 22 administrative divisions of Guatamala City.</obo:IAO_0000115>
        <oboInOwl:hasOBONamespace>GAZ</oboInOwl:hasOBONamespace>
        <oboInOwl:id>GAZ:00248540</oboInOwl:id>
        <rdfs:label>Zone 6</rdfs:label>
    </owl:NamedIndividual>
    


    <!-- http://purl.obolibrary.org/obo/GAZ_00248541 -->

    <owl:NamedIndividual rdf:about="http://purl.obolibrary.org/obo/GAZ_00248541">
        <obo:RO_0001025 rdf:resource="http://purl.obolibrary.org/obo/GAZ_00005154"/>
        <obo:IAO_0000115>One of the 22 administrative divisions of Guatamala City.</obo:IAO_0000115>
        <oboInOwl:hasOBONamespace>GAZ</oboInOwl:hasOBONamespace>
        <oboInOwl:id>GAZ:00248541</oboInOwl:id>
        <rdfs:label>Zone 7</rdfs:label>
    </owl:NamedIndividual>
    


    <!-- http://purl.obolibrary.org/obo/GAZ_00248542 -->

    <owl:NamedIndividual rdf:about="http://purl.obolibrary.org/obo/GAZ_00248542">
        <obo:RO_0001025 rdf:resource="http://purl.obolibrary.org/obo/GAZ_00005154"/>
        <obo:IAO_0000115>One of the 22 administrative divisions of Guatamala City.</obo:IAO_0000115>
        <oboInOwl:hasOBONamespace>GAZ</oboInOwl:hasOBONamespace>
        <oboInOwl:id>GAZ:00248542</oboInOwl:id>
        <rdfs:label>Zone 8</rdfs:label>
    </owl:NamedIndividual>
    


    <!-- http://purl.obolibrary.org/obo/GAZ_00248543 -->

    <owl:NamedIndividual rdf:about="http://purl.obolibrary.org/obo/GAZ_00248543">
        <obo:RO_0001025 rdf:resource="http://purl.obolibrary.org/obo/GAZ_00005154"/>
        <obo:IAO_0000115>One of the 22 administrative divisions of Guatamala City.</obo:IAO_0000115>
        <oboInOwl:hasOBONamespace>GAZ</oboInOwl:hasOBONamespace>
        <oboInOwl:id>GAZ:00248543</oboInOwl:id>
        <rdfs:label>Zone 9</rdfs:label>
    </owl:NamedIndividual>
    


    <!-- http://purl.obolibrary.org/obo/GAZ_00248544 -->

    <owl:NamedIndividual rdf:about="http://purl.obolibrary.org/obo/GAZ_00248544">
        <obo:RO_0001025 rdf:resource="http://purl.obolibrary.org/obo/GAZ_00005154"/>
        <obo:IAO_0000115>One of the 22 administrative divisions of Guatamala City.</obo:IAO_0000115>
        <oboInOwl:hasOBONamespace>GAZ</oboInOwl:hasOBONamespace>
        <oboInOwl:id>GAZ:00248544</oboInOwl:id>
        <rdfs:label>Zone 10</rdfs:label>
    </owl:NamedIndividual>
    


    <!-- http://purl.obolibrary.org/obo/GAZ_00248545 -->

    <owl:NamedIndividual rdf:about="http://purl.obolibrary.org/obo/GAZ_00248545">
        <obo:RO_0001025 rdf:resource="http://purl.obolibrary.org/obo/GAZ_00005154"/>
        <obo:IAO_0000115>One of the 22 administrative divisions of Guatamala City.</obo:IAO_0000115>
        <oboInOwl:hasOBONamespace>GAZ</oboInOwl:hasOBONamespace>
        <oboInOwl:id>GAZ:00248545</oboInOwl:id>
        <rdfs:label>Zone 11</rdfs:label>
    </owl:NamedIndividual>
    


    <!-- http://purl.obolibrary.org/obo/GAZ_00248546 -->

    <owl:NamedIndividual rdf:about="http://purl.obolibrary.org/obo/GAZ_00248546">
        <obo:RO_0001025 rdf:resource="http://purl.obolibrary.org/obo/GAZ_00005154"/>
        <obo:IAO_0000115>One of the 22 administrative divisions of Guatamala City.</obo:IAO_0000115>
        <oboInOwl:hasOBONamespace>GAZ</oboInOwl:hasOBONamespace>
        <oboInOwl:id>GAZ:00248546</oboInOwl:id>
        <rdfs:label>Zone 12</rdfs:label>
    </owl:NamedIndividual>
    


    <!-- http://purl.obolibrary.org/obo/GAZ_00248547 -->

    <owl:NamedIndividual rdf:about="http://purl.obolibrary.org/obo/GAZ_00248547">
        <obo:RO_0001025 rdf:resource="http://purl.obolibrary.org/obo/GAZ_00005154"/>
        <obo:IAO_0000115>One of the 22 administrative divisions of Guatamala City.</obo:IAO_0000115>
        <oboInOwl:hasOBONamespace>GAZ</oboInOwl:hasOBONamespace>
        <oboInOwl:id>GAZ:00248547</oboInOwl:id>
        <rdfs:label>Zone 13</rdfs:label>
    </owl:NamedIndividual>
    


    <!-- http://purl.obolibrary.org/obo/GAZ_00248548 -->

    <owl:NamedIndividual rdf:about="http://purl.obolibrary.org/obo/GAZ_00248548">
        <obo:RO_0001025 rdf:resource="http://purl.obolibrary.org/obo/GAZ_00005154"/>
        <obo:IAO_0000115>One of the 22 administrative divisions of Guatamala City.</obo:IAO_0000115>
        <oboInOwl:hasOBONamespace>GAZ</oboInOwl:hasOBONamespace>
        <oboInOwl:id>GAZ:00248548</oboInOwl:id>
        <rdfs:label>Zone 14</rdfs:label>
    </owl:NamedIndividual>
    


    <!-- http://purl.obolibrary.org/obo/GAZ_00248549 -->

    <owl:NamedIndividual rdf:about="http://purl.obolibrary.org/obo/GAZ_00248549">
        <obo:RO_0001025 rdf:resource="http://purl.obolibrary.org/obo/GAZ_00005154"/>
        <obo:IAO_0000115>One of the 22 administrative divisions of Guatamala City.</obo:IAO_0000115>
        <oboInOwl:hasOBONamespace>GAZ</oboInOwl:hasOBONamespace>
        <oboInOwl:id>GAZ:00248549</oboInOwl:id>
        <rdfs:label>Zone 15</rdfs:label>
    </owl:NamedIndividual>
    


    <!-- http://purl.obolibrary.org/obo/GAZ_00248550 -->

    <owl:NamedIndividual rdf:about="http://purl.obolibrary.org/obo/GAZ_00248550">
        <obo:RO_0001025 rdf:resource="http://purl.obolibrary.org/obo/GAZ_00005154"/>
        <obo:IAO_0000115>One of the 22 administrative divisions of Guatamala City.</obo:IAO_0000115>
        <oboInOwl:hasOBONamespace>GAZ</oboInOwl:hasOBONamespace>
        <oboInOwl:id>GAZ:00248550</oboInOwl:id>
        <rdfs:label>Zone 16</rdfs:label>
    </owl:NamedIndividual>
    


    <!-- http://purl.obolibrary.org/obo/GAZ_00248551 -->

    <owl:NamedIndividual rdf:about="http://purl.obolibrary.org/obo/GAZ_00248551">
        <obo:RO_0001025 rdf:resource="http://purl.obolibrary.org/obo/GAZ_00005154"/>
        <obo:IAO_0000115>One of the 22 administrative divisions of Guatamala City.</obo:IAO_0000115>
        <oboInOwl:hasOBONamespace>GAZ</oboInOwl:hasOBONamespace>
        <oboInOwl:id>GAZ:00248551</oboInOwl:id>
        <rdfs:label>Zone 17</rdfs:label>
    </owl:NamedIndividual>
    


    <!-- http://purl.obolibrary.org/obo/GAZ_00248552 -->

    <owl:NamedIndividual rdf:about="http://purl.obolibrary.org/obo/GAZ_00248552">
        <obo:RO_0001025 rdf:resource="http://purl.obolibrary.org/obo/GAZ_00005154"/>
        <obo:IAO_0000115>One of the 22 administrative divisions of Guatamala City.</obo:IAO_0000115>
        <oboInOwl:hasOBONamespace>GAZ</oboInOwl:hasOBONamespace>
        <oboInOwl:id>GAZ:00248552</oboInOwl:id>
        <rdfs:label>Zone 18</rdfs:label>
    </owl:NamedIndividual>
    


    <!-- http://purl.obolibrary.org/obo/GAZ_00248553 -->

    <owl:NamedIndividual rdf:about="http://purl.obolibrary.org/obo/GAZ_00248553">
        <obo:RO_0001025 rdf:resource="http://purl.obolibrary.org/obo/GAZ_00005154"/>
        <obo:IAO_0000115>One of the 22 administrative divisions of Guatamala City.</obo:IAO_0000115>
        <oboInOwl:hasOBONamespace>GAZ</oboInOwl:hasOBONamespace>
        <oboInOwl:id>GAZ:00248553</oboInOwl:id>
        <rdfs:label>Zone 19</rdfs:label>
    </owl:NamedIndividual>
    


    <!-- http://purl.obolibrary.org/obo/GAZ_00248554 -->

    <owl:NamedIndividual rdf:about="http://purl.obolibrary.org/obo/GAZ_00248554">
        <obo:RO_0001025 rdf:resource="http://purl.obolibrary.org/obo/GAZ_00005154"/>
        <obo:IAO_0000115>One of the 22 administrative divisions of Guatamala City.</obo:IAO_0000115>
        <oboInOwl:hasOBONamespace>GAZ</oboInOwl:hasOBONamespace>
        <oboInOwl:id>GAZ:00248554</oboInOwl:id>
        <rdfs:label>Zone 21</rdfs:label>
    </owl:NamedIndividual>
    


    <!-- http://purl.obolibrary.org/obo/GAZ_00248555 -->

    <owl:NamedIndividual rdf:about="http://purl.obolibrary.org/obo/GAZ_00248555">
        <obo:RO_0001025 rdf:resource="http://purl.obolibrary.org/obo/GAZ_00005154"/>
        <obo:IAO_0000115>One of the 22 administrative divisions of Guatamala City.</obo:IAO_0000115>
        <oboInOwl:hasOBONamespace>GAZ</oboInOwl:hasOBONamespace>
        <oboInOwl:id>GAZ:00248555</oboInOwl:id>
        <rdfs:label>Zone 24</rdfs:label>
    </owl:NamedIndividual>
    


    <!-- http://purl.obolibrary.org/obo/GAZ_00248556 -->

    <owl:NamedIndividual rdf:about="http://purl.obolibrary.org/obo/GAZ_00248556">
        <obo:RO_0001025 rdf:resource="http://purl.obolibrary.org/obo/GAZ_00005154"/>
        <obo:IAO_0000115>One of the 22 administrative divisions of Guatamala City.</obo:IAO_0000115>
        <oboInOwl:hasOBONamespace>GAZ</oboInOwl:hasOBONamespace>
        <oboInOwl:id>GAZ:00248556</oboInOwl:id>
        <rdfs:label>Zone 25</rdfs:label>
    </owl:NamedIndividual>
    


    <!-- http://purl.obolibrary.org/obo/GAZ_00248557 -->

    <owl:NamedIndividual rdf:about="http://purl.obolibrary.org/obo/GAZ_00248557">
        <obo:RO_0001025 rdf:resource="http://purl.obolibrary.org/obo/GAZ_00005155"/>
        <obo:IAO_0000115>A freshwater lake located close to the south of Guatemala City at an altitude of 1,188 m above sea level. The lake consists of two basins connected by a narrow constriction, where a dry dock was constructed to let the railway pass through. This separated the lake into two water bodies with different physical, chemical and biological characteristics. The lake&apos;s primary inflow is the Villalobos River, and the lake is drained by the Michatoya River, an important tributary of the Maria Linda River.</obo:IAO_0000115>
        <oboInOwl:hasOBONamespace>GAZ</oboInOwl:hasOBONamespace>
        <oboInOwl:id>GAZ:00248557</oboInOwl:id>
        <rdfs:label>Laguna de Amatitlan</rdfs:label>
    </owl:NamedIndividual>
    


    <!-- http://purl.obolibrary.org/obo/GAZ_00248558 -->

    <owl:NamedIndividual rdf:about="http://purl.obolibrary.org/obo/GAZ_00248558">
        <obo:RO_0001025 rdf:resource="http://purl.obolibrary.org/obo/GAZ_00068136"/>
        <obo:IAO_0000115>A freshwater lake. Located on the border with Mexico, 80 km N of Huehuetenango.</obo:IAO_0000115>
        <oboInOwl:hasOBONamespace>GAZ</oboInOwl:hasOBONamespace>
        <oboInOwl:id>GAZ:00248558</oboInOwl:id>
        <rdfs:label>Laguna de Yolnabaj</rdfs:label>
    </owl:NamedIndividual>
    


    <!-- http://purl.obolibrary.org/obo/GAZ_00248559 -->

    <owl:NamedIndividual rdf:about="http://purl.obolibrary.org/obo/GAZ_00248559">
        <obo:RO_0001025 rdf:resource="http://purl.obolibrary.org/obo/GAZ_00000494"/>
        <obo:IAO_0000115>Seasonal marshes and wetlands on the floodplain of the Rio Polochic. Located W of Lago de Izabal.</obo:IAO_0000115>
        <oboInOwl:hasOBONamespace>GAZ</oboInOwl:hasOBONamespace>
        <oboInOwl:id>GAZ:00248559</oboInOwl:id>
        <rdfs:label>Bujajal-Polichic Marshes</rdfs:label>
    </owl:NamedIndividual>
    


    <!-- http://purl.obolibrary.org/obo/GAZ_00248560 -->

    <owl:NamedIndividual rdf:about="http://purl.obolibrary.org/obo/GAZ_00248560">
        <obo:RO_0001025 rdf:resource="http://purl.obolibrary.org/obo/GAZ_00000494"/>
        <obo:IAO_0000115>A river draining Lago de Izabel ot the Caribbean.</obo:IAO_0000115>
        <oboInOwl:hasOBONamespace>GAZ</oboInOwl:hasOBONamespace>
        <oboInOwl:id>GAZ:00248560</oboInOwl:id>
        <rdfs:label>Golfete Dulce</rdfs:label>
    </owl:NamedIndividual>
    


    <!-- http://purl.obolibrary.org/obo/GAZ_00248562 -->

    <owl:NamedIndividual rdf:about="http://purl.obolibrary.org/obo/GAZ_00248562">
        <obo:RO_0001025 rdf:resource="http://purl.obolibrary.org/obo/GAZ_00248560"/>
        <obo:IAO_0000115>A lake-like section of the Golfete Duce.</obo:IAO_0000115>
        <oboInOwl:hasOBONamespace>GAZ</oboInOwl:hasOBONamespace>
        <oboInOwl:id>GAZ:00248562</oboInOwl:id>
        <rdfs:label>Golfete</rdfs:label>
    </owl:NamedIndividual>
    


    <!-- http://purl.obolibrary.org/obo/GAZ_00248563 -->

    <owl:NamedIndividual rdf:about="http://purl.obolibrary.org/obo/GAZ_00248563">
        <obo:RO_0001025 rdf:resource="http://purl.obolibrary.org/obo/GAZ_00000494"/>
        <obo:IAO_0000115>A river draining Lago de Izabal to the Caribbean.</obo:IAO_0000115>
        <oboInOwl:hasOBONamespace>GAZ</oboInOwl:hasOBONamespace>
        <oboInOwl:id>GAZ:00248563</oboInOwl:id>
        <rdfs:label>Rio Dulce</rdfs:label>
    </owl:NamedIndividual>
    


    <!-- http://purl.obolibrary.org/obo/GAZ_00248565 -->

    <owl:NamedIndividual rdf:about="http://purl.obolibrary.org/obo/GAZ_00248565">
        <obo:RO_0001025 rdf:resource="http://purl.obolibrary.org/obo/GAZ_00000494"/>
        <obo:IAO_0000115>Brackish marhses on the E shore of Bahia de Amatique. Located N pf Puerto Barrios.</obo:IAO_0000115>
        <oboInOwl:hasOBONamespace>GAZ</oboInOwl:hasOBONamespace>
        <oboInOwl:id>GAZ:00248565</oboInOwl:id>
        <rdfs:label>La Graciosa Marhses</rdfs:label>
    </owl:NamedIndividual>
    


    <!-- http://purl.obolibrary.org/obo/GAZ_00248566 -->

    <owl:NamedIndividual rdf:about="http://purl.obolibrary.org/obo/GAZ_00248566">
        <obo:RO_0001025 rdf:resource="http://purl.obolibrary.org/obo/GAZ_00000430"/>
        <obo:IAO_0000115>A freshwater lake. Located 85 km W of El Achiotal.</obo:IAO_0000115>
        <oboInOwl:hasOBONamespace>GAZ</oboInOwl:hasOBONamespace>
        <oboInOwl:id>GAZ:00248566</oboInOwl:id>
        <rdfs:label>Laguna de Lachwa</rdfs:label>
    </owl:NamedIndividual>
    


    <!-- http://purl.obolibrary.org/obo/GAZ_00248567 -->

    <owl:NamedIndividual rdf:about="http://purl.obolibrary.org/obo/GAZ_00248567">
        <obo:RO_0001025 rdf:resource="http://purl.obolibrary.org/obo/GAZ_00000508"/>
        <obo:IAO_0000115>A freshwater lake. Located W of Sayaxche.</obo:IAO_0000115>
        <oboInOwl:hasOBONamespace>GAZ</oboInOwl:hasOBONamespace>
        <oboInOwl:id>GAZ:00248567</oboInOwl:id>
        <rdfs:label>Laguna Petexbatun</rdfs:label>
    </owl:NamedIndividual>
    


    <!-- http://purl.obolibrary.org/obo/GAZ_00248568 -->

    <owl:NamedIndividual rdf:about="http://purl.obolibrary.org/obo/GAZ_00248568">
        <obo:RO_0001025 rdf:resource="http://purl.obolibrary.org/obo/GAZ_00000508"/>
        <obo:IAO_0000115>A freshwater lake. Locaated S of Sayaxche.</obo:IAO_0000115>
        <oboInOwl:hasOBONamespace>GAZ</oboInOwl:hasOBONamespace>
        <oboInOwl:id>GAZ:00248568</oboInOwl:id>
        <rdfs:label>Laguna Las Pozas</rdfs:label>
    </owl:NamedIndividual>
    


    <!-- http://purl.obolibrary.org/obo/GAZ_00248569 -->

    <owl:NamedIndividual rdf:about="http://purl.obolibrary.org/obo/GAZ_00248569">
        <obo:RO_0001025 rdf:resource="http://purl.obolibrary.org/obo/GAZ_00000508"/>
        <obo:IAO_0000115>A freshwater lake. Located 30 km ESE of Tixal.</obo:IAO_0000115>
        <oboInOwl:hasOBONamespace>GAZ</oboInOwl:hasOBONamespace>
        <oboInOwl:id>GAZ:00248569</oboInOwl:id>
        <rdfs:label>Laguna Yaxja</rdfs:label>
    </owl:NamedIndividual>
    


    <!-- http://purl.obolibrary.org/obo/GAZ_00248570 -->

    <owl:NamedIndividual rdf:about="http://purl.obolibrary.org/obo/GAZ_00248570">
        <obo:RO_0001025 rdf:resource="http://purl.obolibrary.org/obo/GAZ_00000508"/>
        <obo:IAO_0000115>A freshwater lake. Located 30 km ESE of Tikal.</obo:IAO_0000115>
        <oboInOwl:hasOBONamespace>GAZ</oboInOwl:hasOBONamespace>
        <oboInOwl:id>GAZ:00248570</oboInOwl:id>
        <rdfs:label>Laguna Sachab</rdfs:label>
    </owl:NamedIndividual>
    


    <!-- http://purl.obolibrary.org/obo/GAZ_00248571 -->

    <owl:NamedIndividual rdf:about="http://purl.obolibrary.org/obo/GAZ_00248571">
        <obo:RO_0001025 rdf:resource="http://purl.obolibrary.org/obo/GAZ_00000508"/>
        <obo:IAO_0000115>A freshwater lake. Located 30 km SW of Tikal.</obo:IAO_0000115>
        <oboInOwl:hasOBONamespace>GAZ</oboInOwl:hasOBONamespace>
        <oboInOwl:id>GAZ:00248571</oboInOwl:id>
        <rdfs:label>Laguna Petenchel</rdfs:label>
    </owl:NamedIndividual>
    


    <!-- http://purl.obolibrary.org/obo/GAZ_00248572 -->

    <owl:NamedIndividual rdf:about="http://purl.obolibrary.org/obo/GAZ_00248572">
        <obo:RO_0001025 rdf:resource="http://purl.obolibrary.org/obo/GAZ_00068175"/>
        <obo:IAO_0000115>A freshwater lake. Located 65 km WSW of Tikal.</obo:IAO_0000115>
        <oboInOwl:hasOBONamespace>GAZ</oboInOwl:hasOBONamespace>
        <oboInOwl:id>GAZ:00248572</oboInOwl:id>
        <rdfs:label>Laguna Perdida</rdfs:label>
    </owl:NamedIndividual>
    


    <!-- http://purl.obolibrary.org/obo/GAZ_00248573 -->

    <owl:NamedIndividual rdf:about="http://purl.obolibrary.org/obo/GAZ_00248573">
        <obo:RO_0001025 rdf:resource="http://purl.obolibrary.org/obo/GAZ_00000508"/>
        <obo:IAO_0000115>A wetland. Located 90 km W of Tikal.</obo:IAO_0000115>
        <oboInOwl:hasOBONamespace>GAZ</oboInOwl:hasOBONamespace>
        <oboInOwl:id>GAZ:00248573</oboInOwl:id>
        <rdfs:label>Pantano Los Medanos</rdfs:label>
    </owl:NamedIndividual>
    


    <!-- http://purl.obolibrary.org/obo/GAZ_00248574 -->

    <owl:NamedIndividual rdf:about="http://purl.obolibrary.org/obo/GAZ_00248574">
        <obo:RO_0001025 rdf:resource="http://purl.obolibrary.org/obo/GAZ_00266055"/>
        <obo:IAO_0000115>A freshwater lake. Located 40 km N of El Naranjo.</obo:IAO_0000115>
        <oboInOwl:hasOBONamespace>GAZ</oboInOwl:hasOBONamespace>
        <oboInOwl:id>GAZ:00248574</oboInOwl:id>
        <rdfs:label>Laguna El Tigre</rdfs:label>
    </owl:NamedIndividual>
    


    <!-- http://purl.obolibrary.org/obo/GAZ_00264221 -->

    <owl:NamedIndividual rdf:about="http://purl.obolibrary.org/obo/GAZ_00264221">
        <obo:IAO_0000115>A river in the Toledo District of Belize. It forms the country&apos;s southern boundary with Guatemala. It flows through the Guatemalan departments of Alta Verapaz and Izabal into Belize and through Toledo to the Caribbean Sea.</obo:IAO_0000115>
        <oboInOwl:hasOBONamespace>GAZ</oboInOwl:hasOBONamespace>
        <oboInOwl:id>GAZ:00264221</oboInOwl:id>
        <rdfs:label>Sarstoon River</rdfs:label>
    </owl:NamedIndividual>
    


    <!-- http://purl.obolibrary.org/obo/GAZ_00264226 -->

    <owl:NamedIndividual rdf:about="http://purl.obolibrary.org/obo/GAZ_00264226">
        <obo:IAO_0000115>A river.</obo:IAO_0000115>
        <oboInOwl:hasOBONamespace>GAZ</oboInOwl:hasOBONamespace>
        <oboInOwl:id>GAZ:00264226</oboInOwl:id>
        <rdfs:label>Booth&apos;s River</rdfs:label>
    </owl:NamedIndividual>
    


    <!-- http://purl.obolibrary.org/obo/GAZ_00264241 -->

    <owl:NamedIndividual rdf:about="http://purl.obolibrary.org/obo/GAZ_00264241">
        <obo:RO_0001025 rdf:resource="http://purl.obolibrary.org/obo/GAZ_00000494"/>
        <obo:IAO_0000115>A small peninsula that separates Amatique Bay from the Gulf of Honduras. It is located on Guatemala&apos;s east coast.</obo:IAO_0000115>
        <oboInOwl:hasOBONamespace>GAZ</oboInOwl:hasOBONamespace>
        <oboInOwl:id>GAZ:00264241</oboInOwl:id>
        <rdfs:label>Punta de Manabique</rdfs:label>
    </owl:NamedIndividual>
    


    <!-- http://purl.obolibrary.org/obo/GAZ_00264289 -->

    <owl:NamedIndividual rdf:about="http://purl.obolibrary.org/obo/GAZ_00264289">
        <obo:IAO_0000115>A protected area.</obo:IAO_0000115>
        <oboInOwl:hasOBONamespace>GAZ</oboInOwl:hasOBONamespace>
        <oboInOwl:id>GAZ:00264289</oboInOwl:id>
        <rdfs:label>Columbia River Forest Reserve</rdfs:label>
    </owl:NamedIndividual>
    


    <!-- http://purl.obolibrary.org/obo/GAZ_00265030 -->

    <owl:NamedIndividual rdf:about="http://purl.obolibrary.org/obo/GAZ_00265030">
        <obo:IAO_0000115>A dam that spans the Lempa River 78 km north of San Salvador in the municipalities of Potonico, (Chalatenango) and Jutiapa (Cabanas) in El Salvador.</obo:IAO_0000115>
        <oboInOwl:hasOBONamespace>GAZ</oboInOwl:hasOBONamespace>
        <oboInOwl:id>GAZ:00265030</oboInOwl:id>
        <rdfs:label>Central Hidroelectrica Cerron Grande</rdfs:label>
    </owl:NamedIndividual>
    


    <!-- http://purl.obolibrary.org/obo/GAZ_00265496 -->

    <owl:NamedIndividual rdf:about="http://purl.obolibrary.org/obo/GAZ_00265496">
        <obo:IAO_0000115>An island.</obo:IAO_0000115>
        <oboInOwl:hasOBONamespace>GAZ</oboInOwl:hasOBONamespace>
        <oboInOwl:id>GAZ:00265496</oboInOwl:id>
        <rdfs:label>Teotipa</rdfs:label>
    </owl:NamedIndividual>
    


    <!-- http://purl.obolibrary.org/obo/GAZ_00265497 -->

    <owl:NamedIndividual rdf:about="http://purl.obolibrary.org/obo/GAZ_00265497">
        <obo:IAO_0000115>An island.</obo:IAO_0000115>
        <oboInOwl:hasOBONamespace>GAZ</oboInOwl:hasOBONamespace>
        <oboInOwl:id>GAZ:00265497</oboInOwl:id>
        <rdfs:label>Cerro de Tule</rdfs:label>
    </owl:NamedIndividual>
    


    <!-- http://purl.obolibrary.org/obo/GAZ_00265498 -->

    <owl:NamedIndividual rdf:about="http://purl.obolibrary.org/obo/GAZ_00265498">
        <obo:IAO_0000115>An island.</obo:IAO_0000115>
        <oboInOwl:hasOBONamespace>GAZ</oboInOwl:hasOBONamespace>
        <oboInOwl:id>GAZ:00265498</oboInOwl:id>
        <rdfs:label>Iguatepec</rdfs:label>
    </owl:NamedIndividual>
    


    <!-- http://purl.obolibrary.org/obo/GAZ_00265627 -->

    <owl:NamedIndividual rdf:about="http://purl.obolibrary.org/obo/GAZ_00265627">
        <obo:IAO_0000115>A river.</obo:IAO_0000115>
        <oboInOwl:hasOBONamespace>GAZ</oboInOwl:hasOBONamespace>
        <oboInOwl:id>GAZ:00265627</oboInOwl:id>
        <rdfs:label>Rio Guajoyo</rdfs:label>
    </owl:NamedIndividual>
    


    <!-- http://purl.obolibrary.org/obo/GAZ_00265628 -->

    <owl:NamedIndividual rdf:about="http://purl.obolibrary.org/obo/GAZ_00265628">
        <obo:IAO_0000115>A river.</obo:IAO_0000115>
        <oboInOwl:hasOBONamespace>GAZ</oboInOwl:hasOBONamespace>
        <oboInOwl:id>GAZ:00265628</oboInOwl:id>
        <rdfs:label>Rio Tahuilapa</rdfs:label>
    </owl:NamedIndividual>
    


    <!-- http://purl.obolibrary.org/obo/GAZ_00265638 -->

    <owl:NamedIndividual rdf:about="http://purl.obolibrary.org/obo/GAZ_00265638">
        <obo:IAO_0000115>A river.</obo:IAO_0000115>
        <oboInOwl:hasOBONamespace>GAZ</oboInOwl:hasOBONamespace>
        <oboInOwl:id>GAZ:00265638</oboInOwl:id>
        <rdfs:label>Rio Las Canas</rdfs:label>
    </owl:NamedIndividual>
    


    <!-- http://purl.obolibrary.org/obo/GAZ_00265640 -->

    <owl:NamedIndividual rdf:about="http://purl.obolibrary.org/obo/GAZ_00265640">
        <obo:IAO_0000115>A river.</obo:IAO_0000115>
        <oboInOwl:hasOBONamespace>GAZ</oboInOwl:hasOBONamespace>
        <oboInOwl:id>GAZ:00265640</oboInOwl:id>
        <rdfs:label>Rio Metayate</rdfs:label>
    </owl:NamedIndividual>
    


    <!-- http://purl.obolibrary.org/obo/GAZ_00265641 -->

    <owl:NamedIndividual rdf:about="http://purl.obolibrary.org/obo/GAZ_00265641">
        <obo:IAO_0000115>A river.</obo:IAO_0000115>
        <oboInOwl:hasOBONamespace>GAZ</oboInOwl:hasOBONamespace>
        <oboInOwl:id>GAZ:00265641</oboInOwl:id>
        <rdfs:label>Rio de Grande Tilapa</rdfs:label>
    </owl:NamedIndividual>
    


    <!-- http://purl.obolibrary.org/obo/GAZ_00265642 -->

    <owl:NamedIndividual rdf:about="http://purl.obolibrary.org/obo/GAZ_00265642">
        <obo:IAO_0000115>A river.</obo:IAO_0000115>
        <oboInOwl:hasOBONamespace>GAZ</oboInOwl:hasOBONamespace>
        <oboInOwl:id>GAZ:00265642</oboInOwl:id>
        <rdfs:label>Rio Tamulasco</rdfs:label>
    </owl:NamedIndividual>
    


    <!-- http://purl.obolibrary.org/obo/GAZ_00265652 -->

    <owl:NamedIndividual rdf:about="http://purl.obolibrary.org/obo/GAZ_00265652">
        <obo:IAO_0000115>A river.</obo:IAO_0000115>
        <oboInOwl:hasOBONamespace>GAZ</oboInOwl:hasOBONamespace>
        <oboInOwl:id>GAZ:00265652</oboInOwl:id>
        <rdfs:label>Rio Copinolap</rdfs:label>
    </owl:NamedIndividual>
    


    <!-- http://purl.obolibrary.org/obo/GAZ_00265654 -->

    <owl:NamedIndividual rdf:about="http://purl.obolibrary.org/obo/GAZ_00265654">
        <oboInOwl:hasOBONamespace>GAZ</oboInOwl:hasOBONamespace>
        <oboInOwl:id>GAZ:00265654</oboInOwl:id>
        <rdfs:label>Embalse 15 de Septiembre</rdfs:label>
    </owl:NamedIndividual>
    


    <!-- http://purl.obolibrary.org/obo/GAZ_00265655 -->

    <owl:NamedIndividual rdf:about="http://purl.obolibrary.org/obo/GAZ_00265655">
        <obo:IAO_0000115>A river.</obo:IAO_0000115>
        <oboInOwl:hasOBONamespace>GAZ</oboInOwl:hasOBONamespace>
        <oboInOwl:id>GAZ:00265655</oboInOwl:id>
        <rdfs:label>Rio Machacal</rdfs:label>
    </owl:NamedIndividual>
    


    <!-- http://purl.obolibrary.org/obo/GAZ_00265656 -->

    <owl:NamedIndividual rdf:about="http://purl.obolibrary.org/obo/GAZ_00265656">
        <obo:IAO_0000115>A river.</obo:IAO_0000115>
        <oboInOwl:hasOBONamespace>GAZ</oboInOwl:hasOBONamespace>
        <oboInOwl:id>GAZ:00265656</oboInOwl:id>
        <rdfs:label>Rio Acahuapa</rdfs:label>
    </owl:NamedIndividual>
    


    <!-- http://purl.obolibrary.org/obo/GAZ_00265664 -->

    <owl:NamedIndividual rdf:about="http://purl.obolibrary.org/obo/GAZ_00265664">
        <obo:IAO_0000115>A river.</obo:IAO_0000115>
        <oboInOwl:hasOBONamespace>GAZ</oboInOwl:hasOBONamespace>
        <oboInOwl:id>GAZ:00265664</oboInOwl:id>
        <rdfs:label>Rio El Tamarindo</rdfs:label>
    </owl:NamedIndividual>
    


    <!-- http://purl.obolibrary.org/obo/GAZ_00266009 -->

    <owl:NamedIndividual rdf:about="http://purl.obolibrary.org/obo/GAZ_00266009">
        <obo:RO_0001025 rdf:resource="http://purl.obolibrary.org/obo/GAZ_00000430"/>
        <obo:IAO_0000115>A protected area located in Alta Verapaz, Guatemala, on the north-western outskirts of the city of Coban. Established 1980.</obo:IAO_0000115>
        <oboInOwl:hasOBONamespace>GAZ</oboInOwl:hasOBONamespace>
        <oboInOwl:id>GAZ:00266009</oboInOwl:id>
        <rdfs:label>Parque Nacional Las Victorias</rdfs:label>
    </owl:NamedIndividual>
    


    <!-- http://purl.obolibrary.org/obo/GAZ_00266010 -->

    <owl:NamedIndividual rdf:about="http://purl.obolibrary.org/obo/GAZ_00266010">
        <obo:RO_0001025 rdf:resource="http://purl.obolibrary.org/obo/GAZ_00000430"/>
        <obo:IAO_0000115>A protected area. Located in Alta Verapaz, Guatemala, on the northern outskirts of the city of Coban.</obo:IAO_0000115>
        <oboInOwl:hasOBONamespace>GAZ</oboInOwl:hasOBONamespace>
        <oboInOwl:id>GAZ:00266010</oboInOwl:id>
        <rdfs:label>Parque Nacional San Jose la Colonia</rdfs:label>
    </owl:NamedIndividual>
    


    <!-- http://purl.obolibrary.org/obo/GAZ_00266013 -->

    <owl:NamedIndividual rdf:about="http://purl.obolibrary.org/obo/GAZ_00266013">
        <obo:RO_0001025 rdf:resource="http://purl.obolibrary.org/obo/GAZ_00000430"/>
        <obo:IAO_0000115>A protected area.</obo:IAO_0000115>
        <oboInOwl:hasOBONamespace>GAZ</oboInOwl:hasOBONamespace>
        <oboInOwl:id>GAZ:00266013</oboInOwl:id>
        <rdfs:label>Biotopo Mario Dary Rivera</rdfs:label>
    </owl:NamedIndividual>
    


    <!-- http://purl.obolibrary.org/obo/GAZ_00266014 -->

    <owl:NamedIndividual rdf:about="http://purl.obolibrary.org/obo/GAZ_00266014">
        <obo:RO_0001025 rdf:resource="http://purl.obolibrary.org/obo/GAZ_00068059"/>
        <obo:IAO_0000115>A protected area. Established 1955.</obo:IAO_0000115>
        <oboInOwl:hasOBONamespace>GAZ</oboInOwl:hasOBONamespace>
        <oboInOwl:id>GAZ:00266014</oboInOwl:id>
        <rdfs:label>Parque Nacional Grutas de Lanquin</rdfs:label>
    </owl:NamedIndividual>
    


    <!-- http://purl.obolibrary.org/obo/GAZ_00266015 -->

    <owl:NamedIndividual rdf:about="http://purl.obolibrary.org/obo/GAZ_00266015">
        <obo:RO_0001025 rdf:resource="http://purl.obolibrary.org/obo/GAZ_00266014"/>
        <obo:IAO_0000115>A karst cave.</obo:IAO_0000115>
        <oboInOwl:hasOBONamespace>GAZ</oboInOwl:hasOBONamespace>
        <oboInOwl:id>GAZ:00266015</oboInOwl:id>
        <rdfs:label>Grutas de Lanquin</rdfs:label>
    </owl:NamedIndividual>
    


    <!-- http://purl.obolibrary.org/obo/GAZ_00266017 -->

    <owl:NamedIndividual rdf:about="http://purl.obolibrary.org/obo/GAZ_00266017">
        <rdf:type rdf:resource="http://purl.obolibrary.org/obo/ENVO_00000856"/>
        <obo:RO_0001025 rdf:resource="http://purl.obolibrary.org/obo/GAZ_00000430"/>
        <obo:IAO_0000115>A municipality in the Guatemalan Department of Alta Verapaz.</obo:IAO_0000115>
        <oboInOwl:hasOBONamespace>GAZ</oboInOwl:hasOBONamespace>
        <oboInOwl:id>GAZ:00266017</oboInOwl:id>
        <rdfs:label>Municipality of Raxruha</rdfs:label>
    </owl:NamedIndividual>
    


    <!-- http://purl.obolibrary.org/obo/GAZ_00266018 -->

    <owl:NamedIndividual rdf:about="http://purl.obolibrary.org/obo/GAZ_00266018">
        <obo:RO_0001025 rdf:resource="http://purl.obolibrary.org/obo/GAZ_00068063"/>
        <obo:IAO_0000115>A lake.</obo:IAO_0000115>
        <oboInOwl:hasOBONamespace>GAZ</oboInOwl:hasOBONamespace>
        <oboInOwl:id>GAZ:00266018</oboInOwl:id>
        <rdfs:label>Laguna de Chichoj</rdfs:label>
    </owl:NamedIndividual>
    


    <!-- http://purl.obolibrary.org/obo/GAZ_00266019 -->

    <owl:NamedIndividual rdf:about="http://purl.obolibrary.org/obo/GAZ_00266019">
        <obo:RO_0001025 rdf:resource="http://purl.obolibrary.org/obo/GAZ_00000435"/>
        <obo:IAO_0000115>A protected area.</obo:IAO_0000115>
        <oboInOwl:hasOBONamespace>GAZ</oboInOwl:hasOBONamespace>
        <oboInOwl:id>GAZ:00266019</oboInOwl:id>
        <rdfs:label>Parque Regional Municipal Los Cerritos</rdfs:label>
    </owl:NamedIndividual>
    


    <!-- http://purl.obolibrary.org/obo/GAZ_00266020 -->

    <owl:NamedIndividual rdf:about="http://purl.obolibrary.org/obo/GAZ_00266020">
        <obo:RO_0001025 rdf:resource="http://purl.obolibrary.org/obo/GAZ_00000439"/>
        <obo:IAO_0000115>A Pre-Columbian Mesoamerican archaeological site in the western highlands of Guatemala.</obo:IAO_0000115>
        <oboInOwl:hasOBONamespace>GAZ</oboInOwl:hasOBONamespace>
        <oboInOwl:id>GAZ:00266020</oboInOwl:id>
        <rdfs:label>Iximche</rdfs:label>
    </owl:NamedIndividual>
    


    <!-- http://purl.obolibrary.org/obo/GAZ_00266022 -->

    <owl:NamedIndividual rdf:about="http://purl.obolibrary.org/obo/GAZ_00266022">
        <obo:RO_0001025 rdf:resource="http://purl.obolibrary.org/obo/GAZ_00068081"/>
        <obo:IAO_0000115>A protected area. Established 1987.</obo:IAO_0000115>
        <oboInOwl:hasOBONamespace>GAZ</oboInOwl:hasOBONamespace>
        <oboInOwl:id>GAZ:00266022</oboInOwl:id>
        <rdfs:label>La Reserva de Biosfera Trifinio</rdfs:label>
    </owl:NamedIndividual>
    


    <!-- http://purl.obolibrary.org/obo/GAZ_00266023 -->

    <owl:NamedIndividual rdf:about="http://purl.obolibrary.org/obo/GAZ_00266023">
        <obo:RO_0001025 rdf:resource="http://purl.obolibrary.org/obo/GAZ_00000446"/>
        <obo:IAO_0000115>A protected area.</obo:IAO_0000115>
        <oboInOwl:hasOBONamespace>GAZ</oboInOwl:hasOBONamespace>
        <oboInOwl:id>GAZ:00266023</oboInOwl:id>
        <rdfs:label>Zona de Veda Definitiva Volcan Quezaltepeque</rdfs:label>
    </owl:NamedIndividual>
    


    <!-- http://purl.obolibrary.org/obo/GAZ_00266024 -->

    <owl:NamedIndividual rdf:about="http://purl.obolibrary.org/obo/GAZ_00266024">
        <obo:RO_0001025 rdf:resource="http://purl.obolibrary.org/obo/GAZ_00000446"/>
        <obo:IAO_0000115>A protected area.</obo:IAO_0000115>
        <oboInOwl:hasOBONamespace>GAZ</oboInOwl:hasOBONamespace>
        <oboInOwl:id>GAZ:00266024</oboInOwl:id>
        <rdfs:label>Area de Uso Multiple Volcan y Laguna de Ipala</rdfs:label>
    </owl:NamedIndividual>
    


    <!-- http://purl.obolibrary.org/obo/GAZ_00266025 -->

    <owl:NamedIndividual rdf:about="http://purl.obolibrary.org/obo/GAZ_00266025">
        <obo:RO_0001025 rdf:resource="http://purl.obolibrary.org/obo/GAZ_00056133"/>
        <obo:IAO_0000115>A crater lake.</obo:IAO_0000115>
        <oboInOwl:hasOBONamespace>GAZ</oboInOwl:hasOBONamespace>
        <oboInOwl:id>GAZ:00266025</oboInOwl:id>
        <rdfs:label>Laguna de Ipala</rdfs:label>
    </owl:NamedIndividual>
    


    <!-- http://purl.obolibrary.org/obo/GAZ_00266026 -->

    <owl:NamedIndividual rdf:about="http://purl.obolibrary.org/obo/GAZ_00266026">
        <obo:RO_0001025 rdf:resource="http://purl.obolibrary.org/obo/GAZ_00000476"/>
        <obo:IAO_0000115>A protected area.</obo:IAO_0000115>
        <oboInOwl:hasOBONamespace>GAZ</oboInOwl:hasOBONamespace>
        <oboInOwl:id>GAZ:00266026</oboInOwl:id>
        <rdfs:label>Reserva de la Biosfera de la Sierra de las Minas</rdfs:label>
    </owl:NamedIndividual>
    


    <!-- http://purl.obolibrary.org/obo/GAZ_00266027 -->

    <owl:NamedIndividual rdf:about="http://purl.obolibrary.org/obo/GAZ_00266027">
        <obo:RO_0001025 rdf:resource="http://purl.obolibrary.org/obo/GAZ_00068114"/>
        <obo:IAO_0000115>A major Mesoamerican archaeological site on the Pacific coastal plain of southern Guatemala, belonging to the Maya civilization.</obo:IAO_0000115>
        <oboInOwl:hasOBONamespace>GAZ</oboInOwl:hasOBONamespace>
        <oboInOwl:id>GAZ:00266027</oboInOwl:id>
        <rdfs:label>Balberta</rdfs:label>
    </owl:NamedIndividual>
    


    <!-- http://purl.obolibrary.org/obo/GAZ_00266028 -->

    <owl:NamedIndividual rdf:about="http://purl.obolibrary.org/obo/GAZ_00266028">
        <obo:RO_0001025 rdf:resource="http://purl.obolibrary.org/obo/GAZ_00068107"/>
        <obo:IAO_0000115>A Mesoamerican archaeological site about 1.6 km from the modern town of Santa Lucia Cotzumalguapa in the Escuintla department of Guatemala.</obo:IAO_0000115>
        <oboInOwl:hasOBONamespace>GAZ</oboInOwl:hasOBONamespace>
        <oboInOwl:id>GAZ:00266028</oboInOwl:id>
        <rdfs:label>Bilbao</rdfs:label>
    </owl:NamedIndividual>
    


    <!-- http://purl.obolibrary.org/obo/GAZ_00266029 -->

    <owl:NamedIndividual rdf:about="http://purl.obolibrary.org/obo/GAZ_00266029">
        <obo:RO_0001025 rdf:resource="http://purl.obolibrary.org/obo/GAZ_00068114"/>
        <obo:IAO_0000115>A Mesoamerican archaeological site on the Pacific coastal plain of southern Guatemala. It is located in the department of Escuintla, near Balberta.</obo:IAO_0000115>
        <oboInOwl:hasOBONamespace>GAZ</oboInOwl:hasOBONamespace>
        <oboInOwl:id>GAZ:00266029</oboInOwl:id>
        <rdfs:label>Montana</rdfs:label>
    </owl:NamedIndividual>
    


    <!-- http://purl.obolibrary.org/obo/GAZ_00266031 -->

    <owl:NamedIndividual rdf:about="http://purl.obolibrary.org/obo/GAZ_00266031">
        <obo:RO_0001025 rdf:resource="http://purl.obolibrary.org/obo/GAZ_00068107"/>
        <obo:IAO_0000115>A Pre-Columbian archaeological site in present-day Guatemala.</obo:IAO_0000115>
        <oboInOwl:hasOBONamespace>GAZ</oboInOwl:hasOBONamespace>
        <oboInOwl:id>GAZ:00266031</oboInOwl:id>
        <rdfs:label>El Baul</rdfs:label>
    </owl:NamedIndividual>
    


    <!-- http://purl.obolibrary.org/obo/GAZ_00266032 -->

    <owl:NamedIndividual rdf:about="http://purl.obolibrary.org/obo/GAZ_00266032">
        <obo:RO_0001025 rdf:resource="http://purl.obolibrary.org/obo/GAZ_00068128"/>
        <obo:IAO_0000115>A pre-Columbian Maya archaeological site in the highlands of western Guatemala, about 3.7 km outside of the modern city of Huehuetenango.</obo:IAO_0000115>
        <oboInOwl:hasOBONamespace>GAZ</oboInOwl:hasOBONamespace>
        <oboInOwl:id>GAZ:00266032</oboInOwl:id>
        <rdfs:label>Zaculeu</rdfs:label>
    </owl:NamedIndividual>
    


    <!-- http://purl.obolibrary.org/obo/GAZ_00266034 -->

    <owl:NamedIndividual rdf:about="http://purl.obolibrary.org/obo/GAZ_00266034">
        <obo:RO_0001025 rdf:resource="http://purl.obolibrary.org/obo/GAZ_00000430"/>
        <obo:IAO_0000115>A mountain range. Una pequena cordillera karstica en el norte de Alta Verapaz, Guatemala.</obo:IAO_0000115>
        <oboInOwl:hasOBONamespace>GAZ</oboInOwl:hasOBONamespace>
        <oboInOwl:id>GAZ:00266034</oboInOwl:id>
        <rdfs:label>Sierra de Chinaja</rdfs:label>
    </owl:NamedIndividual>
    


    <!-- http://purl.obolibrary.org/obo/GAZ_00266036 -->

    <owl:NamedIndividual rdf:about="http://purl.obolibrary.org/obo/GAZ_00266036">
        <obo:RO_0001025 rdf:resource="http://purl.obolibrary.org/obo/GAZ_00000483"/>
        <obo:IAO_0000115>A lake.</obo:IAO_0000115>
        <oboInOwl:hasOBONamespace>GAZ</oboInOwl:hasOBONamespace>
        <oboInOwl:id>GAZ:00266036</oboInOwl:id>
        <rdfs:label>Laguna Maxbal</rdfs:label>
    </owl:NamedIndividual>
    


    <!-- http://purl.obolibrary.org/obo/GAZ_00266037 -->

    <owl:NamedIndividual rdf:about="http://purl.obolibrary.org/obo/GAZ_00266037">
        <obo:RO_0001025 rdf:resource="http://purl.obolibrary.org/obo/GAZ_00000483"/>
        <obo:IAO_0000115>A lake.</obo:IAO_0000115>
        <oboInOwl:hasOBONamespace>GAZ</oboInOwl:hasOBONamespace>
        <oboInOwl:id>GAZ:00266037</oboInOwl:id>
        <rdfs:label>Laguna Yolhuitz</rdfs:label>
    </owl:NamedIndividual>
    


    <!-- http://purl.obolibrary.org/obo/GAZ_00266038 -->

    <owl:NamedIndividual rdf:about="http://purl.obolibrary.org/obo/GAZ_00266038">
        <obo:RO_0001025 rdf:resource="http://purl.obolibrary.org/obo/GAZ_00000483"/>
        <obo:IAO_0000115>A lake.</obo:IAO_0000115>
        <oboInOwl:hasOBONamespace>GAZ</oboInOwl:hasOBONamespace>
        <oboInOwl:id>GAZ:00266038</oboInOwl:id>
        <rdfs:label>Laguna Seca</rdfs:label>
    </owl:NamedIndividual>
    


    <!-- http://purl.obolibrary.org/obo/GAZ_00266039 -->

    <owl:NamedIndividual rdf:about="http://purl.obolibrary.org/obo/GAZ_00266039">
        <obo:RO_0001025 rdf:resource="http://purl.obolibrary.org/obo/GAZ_00068139"/>
        <obo:IAO_0000115>An archeological site.</obo:IAO_0000115>
        <oboInOwl:hasOBONamespace>GAZ</oboInOwl:hasOBONamespace>
        <oboInOwl:id>GAZ:00266039</oboInOwl:id>
        <rdfs:label>Yol K&apos;u</rdfs:label>
    </owl:NamedIndividual>
    


    <!-- http://purl.obolibrary.org/obo/GAZ_00266040 -->

    <owl:NamedIndividual rdf:about="http://purl.obolibrary.org/obo/GAZ_00266040">
        <obo:RO_0001025 rdf:resource="http://purl.obolibrary.org/obo/GAZ_00068139"/>
        <obo:IAO_0000115>An archeological site.</obo:IAO_0000115>
        <oboInOwl:hasOBONamespace>GAZ</oboInOwl:hasOBONamespace>
        <oboInOwl:id>GAZ:00266040</oboInOwl:id>
        <rdfs:label>K&apos;atepan</rdfs:label>
    </owl:NamedIndividual>
    


    <!-- http://purl.obolibrary.org/obo/GAZ_00266041 -->

    <owl:NamedIndividual rdf:about="http://purl.obolibrary.org/obo/GAZ_00266041">
        <obo:RO_0001025 rdf:resource="http://purl.obolibrary.org/obo/GAZ_00068139"/>
        <obo:IAO_0000115>An archeological site.</obo:IAO_0000115>
        <oboInOwl:hasOBONamespace>GAZ</oboInOwl:hasOBONamespace>
        <oboInOwl:id>GAZ:00266041</oboInOwl:id>
        <rdfs:label>Curvao</rdfs:label>
    </owl:NamedIndividual>
    


    <!-- http://purl.obolibrary.org/obo/GAZ_00266042 -->

    <owl:NamedIndividual rdf:about="http://purl.obolibrary.org/obo/GAZ_00266042">
        <obo:RO_0001025 rdf:resource="http://purl.obolibrary.org/obo/GAZ_00000494"/>
        <obo:IAO_0000115>A protected area located in the department of Izabal in Guatemala.</obo:IAO_0000115>
        <oboInOwl:hasOBONamespace>GAZ</oboInOwl:hasOBONamespace>
        <oboInOwl:id>GAZ:00266042</oboInOwl:id>
        <rdfs:label>Parque Nacional Rio Dulce</rdfs:label>
    </owl:NamedIndividual>
    


    <!-- http://purl.obolibrary.org/obo/GAZ_00266043 -->

    <owl:NamedIndividual rdf:about="http://purl.obolibrary.org/obo/GAZ_00266043">
        <obo:RO_0001025 rdf:resource="http://purl.obolibrary.org/obo/GAZ_00000494"/>
        <obo:RO_0001025 rdf:resource="http://purl.obolibrary.org/obo/GAZ_00248563"/>
        <obo:IAO_0000115>A long narrow lake in Guatemala. It lies at sea level and is connected by the Dulce River from Lake Izabal draining to the Amatique Bay which is lies in the Caribbean Sea.</obo:IAO_0000115>
        <oboInOwl:hasOBONamespace>GAZ</oboInOwl:hasOBONamespace>
        <oboInOwl:id>GAZ:00266043</oboInOwl:id>
        <rdfs:label>El Golfete</rdfs:label>
    </owl:NamedIndividual>
    


    <!-- http://purl.obolibrary.org/obo/GAZ_00266044 -->

    <owl:NamedIndividual rdf:about="http://purl.obolibrary.org/obo/GAZ_00266044">
        <obo:RO_0001025 rdf:resource="http://purl.obolibrary.org/obo/GAZ_00266054"/>
        <obo:IAO_0000115>A Maya archaeological site in the department of Izabal in south-eastern Guatemala.</obo:IAO_0000115>
        <oboInOwl:hasOBONamespace>GAZ</oboInOwl:hasOBONamespace>
        <oboInOwl:id>GAZ:00266044</oboInOwl:id>
        <rdfs:label>Quirigua</rdfs:label>
    </owl:NamedIndividual>
    


    <!-- http://purl.obolibrary.org/obo/GAZ_00266045 -->

    <owl:NamedIndividual rdf:about="http://purl.obolibrary.org/obo/GAZ_00266045">
        <obo:RO_0001025 rdf:resource="http://purl.obolibrary.org/obo/GAZ_00000494"/>
        <obo:IAO_0000115>A protected area.</obo:IAO_0000115>
        <oboInOwl:hasOBONamespace>GAZ</oboInOwl:hasOBONamespace>
        <oboInOwl:id>GAZ:00266045</oboInOwl:id>
        <rdfs:label>El Refugio de Vida Silvestre Punta de Manabique</rdfs:label>
    </owl:NamedIndividual>
    


    <!-- http://purl.obolibrary.org/obo/GAZ_00266046 -->

    <owl:NamedIndividual rdf:about="http://purl.obolibrary.org/obo/GAZ_00266046">
        <obo:RO_0001025 rdf:resource="http://purl.obolibrary.org/obo/GAZ_00000494"/>
        <obo:IAO_0000115>A protected area.</obo:IAO_0000115>
        <oboInOwl:hasOBONamespace>GAZ</oboInOwl:hasOBONamespace>
        <oboInOwl:id>GAZ:00266046</oboInOwl:id>
        <rdfs:label>La Reserva de la Biosfera de las Minas</rdfs:label>
    </owl:NamedIndividual>
    


    <!-- http://purl.obolibrary.org/obo/GAZ_00266047 -->

    <owl:NamedIndividual rdf:about="http://purl.obolibrary.org/obo/GAZ_00266047">
        <obo:RO_0001025 rdf:resource="http://purl.obolibrary.org/obo/GAZ_00000494"/>
        <obo:IAO_0000115>A protected area.</obo:IAO_0000115>
        <oboInOwl:hasOBONamespace>GAZ</oboInOwl:hasOBONamespace>
        <oboInOwl:id>GAZ:00266047</oboInOwl:id>
        <rdfs:label>El Parque Nacional Bahia de Santo Tomas</rdfs:label>
    </owl:NamedIndividual>
    


    <!-- http://purl.obolibrary.org/obo/GAZ_00266048 -->

    <owl:NamedIndividual rdf:about="http://purl.obolibrary.org/obo/GAZ_00266048">
        <obo:RO_0001025 rdf:resource="http://purl.obolibrary.org/obo/GAZ_00000494"/>
        <obo:IAO_0000115>A protected area.</obo:IAO_0000115>
        <oboInOwl:hasOBONamespace>GAZ</oboInOwl:hasOBONamespace>
        <oboInOwl:id>GAZ:00266048</oboInOwl:id>
        <rdfs:label>La Reserva Protectora de Manantiales Cerro San Gil</rdfs:label>
    </owl:NamedIndividual>
    


    <!-- http://purl.obolibrary.org/obo/GAZ_00266049 -->

    <owl:NamedIndividual rdf:about="http://purl.obolibrary.org/obo/GAZ_00266049">
        <obo:RO_0001025 rdf:resource="http://purl.obolibrary.org/obo/GAZ_00000494"/>
        <obo:IAO_0000115>A protected area.</obo:IAO_0000115>
        <oboInOwl:hasOBONamespace>GAZ</oboInOwl:hasOBONamespace>
        <oboInOwl:id>GAZ:00266049</oboInOwl:id>
        <rdfs:label>La Reserva Biologica de Rio Dulce</rdfs:label>
    </owl:NamedIndividual>
    


    <!-- http://purl.obolibrary.org/obo/GAZ_00266050 -->

    <owl:NamedIndividual rdf:about="http://purl.obolibrary.org/obo/GAZ_00266050">
        <obo:RO_0001025 rdf:resource="http://purl.obolibrary.org/obo/GAZ_00068150"/>
        <obo:IAO_0000115>A protected nature reserve in eastern Guatemala.</obo:IAO_0000115>
        <oboInOwl:hasOBONamespace>GAZ</oboInOwl:hasOBONamespace>
        <oboInOwl:id>GAZ:00266050</oboInOwl:id>
        <rdfs:label>El Biotopo protegido del Manati Chocon Machacas</rdfs:label>
    </owl:NamedIndividual>
    


    <!-- http://purl.obolibrary.org/obo/GAZ_00266051 -->

    <owl:NamedIndividual rdf:about="http://purl.obolibrary.org/obo/GAZ_00266051">
        <obo:RO_0001025 rdf:resource="http://purl.obolibrary.org/obo/GAZ_00000494"/>
        <obo:IAO_0000115>A protected area.</obo:IAO_0000115>
        <oboInOwl:hasOBONamespace>GAZ</oboInOwl:hasOBONamespace>
        <oboInOwl:id>GAZ:00266051</oboInOwl:id>
        <rdfs:label>Reserva Natural Privada el Higuerito</rdfs:label>
    </owl:NamedIndividual>
    


    <!-- http://purl.obolibrary.org/obo/GAZ_00266052 -->

    <owl:NamedIndividual rdf:about="http://purl.obolibrary.org/obo/GAZ_00266052">
        <obo:RO_0001025 rdf:resource="http://purl.obolibrary.org/obo/GAZ_00000494"/>
        <obo:IAO_0000115>A protected area.</obo:IAO_0000115>
        <oboInOwl:hasOBONamespace>GAZ</oboInOwl:hasOBONamespace>
        <oboInOwl:id>GAZ:00266052</oboInOwl:id>
        <rdfs:label>La Reserva Natural privada Rio Blanco</rdfs:label>
    </owl:NamedIndividual>
    


    <!-- http://purl.obolibrary.org/obo/GAZ_00266053 -->

    <owl:NamedIndividual rdf:about="http://purl.obolibrary.org/obo/GAZ_00266053">
        <obo:RO_0001025 rdf:resource="http://purl.obolibrary.org/obo/GAZ_00000494"/>
        <obo:IAO_0000115>A protected area.</obo:IAO_0000115>
        <oboInOwl:hasOBONamespace>GAZ</oboInOwl:hasOBONamespace>
        <oboInOwl:id>GAZ:00266053</oboInOwl:id>
        <rdfs:label>El Refugio de Vida Silvestre Bocas del Polochic</rdfs:label>
    </owl:NamedIndividual>
    


    <!-- http://purl.obolibrary.org/obo/GAZ_00266054 -->

    <owl:NamedIndividual rdf:about="http://purl.obolibrary.org/obo/GAZ_00266054">
        <obo:RO_0001025 rdf:resource="http://purl.obolibrary.org/obo/GAZ_00068153"/>
        <obo:IAO_0000115>A protected area.</obo:IAO_0000115>
        <oboInOwl:hasOBONamespace>GAZ</oboInOwl:hasOBONamespace>
        <oboInOwl:id>GAZ:00266054</oboInOwl:id>
        <rdfs:label>Monumento Natural Quirigua</rdfs:label>
    </owl:NamedIndividual>
    


    <!-- http://purl.obolibrary.org/obo/GAZ_00266055 -->

    <owl:NamedIndividual rdf:about="http://purl.obolibrary.org/obo/GAZ_00266055">
        <obo:RO_0001025 rdf:resource="http://purl.obolibrary.org/obo/GAZ_00000508"/>
        <obo:IAO_0000115>A protected area.</obo:IAO_0000115>
        <oboInOwl:hasOBONamespace>GAZ</oboInOwl:hasOBONamespace>
        <oboInOwl:id>GAZ:00266055</oboInOwl:id>
        <rdfs:label>Parque Nacional Laguna El Tigre</rdfs:label>
    </owl:NamedIndividual>
    


    <!-- http://purl.obolibrary.org/obo/GAZ_00266056 -->

    <owl:NamedIndividual rdf:about="http://purl.obolibrary.org/obo/GAZ_00266056">
        <obo:RO_0001025 rdf:resource="http://purl.obolibrary.org/obo/GAZ_00000499"/>
        <obo:IAO_0000115>A lake.</obo:IAO_0000115>
        <oboInOwl:hasOBONamespace>GAZ</oboInOwl:hasOBONamespace>
        <oboInOwl:id>GAZ:00266056</oboInOwl:id>
        <rdfs:label>Laguna de Atescatempa</rdfs:label>
    </owl:NamedIndividual>
    


    <!-- http://purl.obolibrary.org/obo/GAZ_00266057 -->

    <owl:NamedIndividual rdf:about="http://purl.obolibrary.org/obo/GAZ_00266057">
        <obo:RO_0001025 rdf:resource="http://purl.obolibrary.org/obo/GAZ_00000509"/>
        <obo:IAO_0000115>A Pre-Columbian archeoogical site of the Maya civilization located in the Department of Peten, Guatemala.</obo:IAO_0000115>
        <oboInOwl:hasOBONamespace>GAZ</oboInOwl:hasOBONamespace>
        <oboInOwl:id>GAZ:00266057</oboInOwl:id>
        <rdfs:label>Dos Pilas</rdfs:label>
    </owl:NamedIndividual>
    


    <!-- http://purl.obolibrary.org/obo/GAZ_00266058 -->

    <owl:NamedIndividual rdf:about="http://purl.obolibrary.org/obo/GAZ_00266058">
        <obo:RO_0001025 rdf:resource="http://purl.obolibrary.org/obo/GAZ_00266060"/>
        <obo:IAO_0000115>A Maya archaeological site in the northern Peten region of Guatemala, about 25 km northeast of the modern-day settlement of Carmelita.</obo:IAO_0000115>
        <oboInOwl:hasOBONamespace>GAZ</oboInOwl:hasOBONamespace>
        <oboInOwl:id>GAZ:00266058</oboInOwl:id>
        <rdfs:label>El Tintal</rdfs:label>
    </owl:NamedIndividual>
    


    <!-- http://purl.obolibrary.org/obo/GAZ_00266059 -->

    <owl:NamedIndividual rdf:about="http://purl.obolibrary.org/obo/GAZ_00266059">
        <obo:RO_0001025 rdf:resource="http://purl.obolibrary.org/obo/GAZ_00266060"/>
        <obo:IAO_0000115>A pre-Columbian Mayan archeological site, located in the north of the modern department of El Peten, Guatemala.</obo:IAO_0000115>
        <oboInOwl:hasOBONamespace>GAZ</oboInOwl:hasOBONamespace>
        <oboInOwl:id>GAZ:00266059</oboInOwl:id>
        <rdfs:label>El Mirador</rdfs:label>
    </owl:NamedIndividual>
    


    <!-- http://purl.obolibrary.org/obo/GAZ_00266060 -->

    <owl:NamedIndividual rdf:about="http://purl.obolibrary.org/obo/GAZ_00266060">
        <obo:RO_0001025 rdf:resource="http://purl.obolibrary.org/obo/GAZ_00000508"/>
        <obo:IAO_0000115>A geographically defined elevated basin found in the remote rain forest of the northern Department of Peten, Guatemala. The basin is dominated by low lying swamps called bajos. The basin is surrounded by rugged karstic limestone hills on the east, south, and to a lesser degree, the western side, forming a triangular geographical trough covering more than 2169 km2.</obo:IAO_0000115>
        <oboInOwl:hasOBONamespace>GAZ</oboInOwl:hasOBONamespace>
        <oboInOwl:id>GAZ:00266060</oboInOwl:id>
        <rdfs:label>Mirador Basin</rdfs:label>
    </owl:NamedIndividual>
    


    <!-- http://purl.obolibrary.org/obo/GAZ_00266061 -->

    <owl:NamedIndividual rdf:about="http://purl.obolibrary.org/obo/GAZ_00266061">
        <obo:RO_0001025 rdf:resource="http://purl.obolibrary.org/obo/GAZ_00266060"/>
        <obo:IAO_0000115>An early Maya archaeological site. Nakbe is located in the Mirador Basin, in El Peten region of Guatemala, approximately 13 km south of the Largest Maya city of El Mirador.</obo:IAO_0000115>
        <oboInOwl:hasOBONamespace>GAZ</oboInOwl:hasOBONamespace>
        <oboInOwl:id>GAZ:00266061</oboInOwl:id>
        <rdfs:label>Nakbe</rdfs:label>
    </owl:NamedIndividual>
    


    <!-- http://purl.obolibrary.org/obo/GAZ_00266062 -->

    <owl:NamedIndividual rdf:about="http://purl.obolibrary.org/obo/GAZ_00266062">
        <obo:RO_0001025 rdf:resource="http://purl.obolibrary.org/obo/GAZ_00000508"/>
        <obo:IAO_0000115>A geographical subregion of Mesoamerica, located in the northern portion of the modern-day nation of Guatemala, and essentially contained within the Department of El Peten.</obo:IAO_0000115>
        <oboInOwl:hasOBONamespace>GAZ</oboInOwl:hasOBONamespace>
        <oboInOwl:id>GAZ:00266062</oboInOwl:id>
        <rdfs:label>Peten Basin</rdfs:label>
    </owl:NamedIndividual>
    


    <!-- http://purl.obolibrary.org/obo/GAZ_00266063 -->

    <owl:NamedIndividual rdf:about="http://purl.obolibrary.org/obo/GAZ_00266063">
        <obo:RO_0001025 rdf:resource="http://purl.obolibrary.org/obo/GAZ_00266062"/>
        <obo:IAO_0000115>An archeological site. An ancient ruin of the Maya civilization, located in the Peten Basin region of the Maya lowlands, in the present-day department of Peten, Guatemala. The site lies some 19 km north of the major center of Tikal.</obo:IAO_0000115>
        <oboInOwl:hasOBONamespace>GAZ</oboInOwl:hasOBONamespace>
        <oboInOwl:id>GAZ:00266063</oboInOwl:id>
        <rdfs:label>Uaxactun</rdfs:label>
    </owl:NamedIndividual>
    


    <!-- http://purl.obolibrary.org/obo/GAZ_00266064 -->

    <owl:NamedIndividual rdf:about="http://purl.obolibrary.org/obo/GAZ_00266064">
        <obo:RO_0001025 rdf:resource="http://purl.obolibrary.org/obo/GAZ_00266078"/>
        <obo:IAO_0000115>An archeological site. One of the largest archaeological sites and urban centres of the pre-Columbian Maya civilization. It is located in the archaeological region of the Peten Basin in what is now modern-day northern Guatemala.</obo:IAO_0000115>
        <oboInOwl:hasOBONamespace>GAZ</oboInOwl:hasOBONamespace>
        <oboInOwl:id>GAZ:00266064</oboInOwl:id>
        <rdfs:label>Tikal</rdfs:label>
    </owl:NamedIndividual>
    


    <!-- http://purl.obolibrary.org/obo/GAZ_00266065 -->

    <owl:NamedIndividual rdf:about="http://purl.obolibrary.org/obo/GAZ_00266065">
        <obo:RO_0001025 rdf:resource="http://purl.obolibrary.org/obo/GAZ_00266062"/>
        <obo:IAO_0000115>A pre-Columbian archaeological site of the Maya civilization, located in the northeastern Peten Basin region in Guatemala, near the modern-day border with Belize.</obo:IAO_0000115>
        <oboInOwl:hasOBONamespace>GAZ</oboInOwl:hasOBONamespace>
        <oboInOwl:id>GAZ:00266065</oboInOwl:id>
        <rdfs:label>Holmul</rdfs:label>
    </owl:NamedIndividual>
    


    <!-- http://purl.obolibrary.org/obo/GAZ_00266066 -->

    <owl:NamedIndividual rdf:about="http://purl.obolibrary.org/obo/GAZ_00266066">
        <obo:RO_0001025 rdf:resource="http://purl.obolibrary.org/obo/GAZ_00266062"/>
        <obo:IAO_0000115>An archaeological site of the pre-Columbian Maya civilization, located in the Peten Basin region of present-day Guatemala.</obo:IAO_0000115>
        <oboInOwl:hasOBONamespace>GAZ</oboInOwl:hasOBONamespace>
        <oboInOwl:id>GAZ:00266066</oboInOwl:id>
        <rdfs:label>La Sufricaya</rdfs:label>
    </owl:NamedIndividual>
    


    <!-- http://purl.obolibrary.org/obo/GAZ_00266067 -->

    <owl:NamedIndividual rdf:about="http://purl.obolibrary.org/obo/GAZ_00266067">
        <obo:RO_0001025 rdf:resource="http://purl.obolibrary.org/obo/GAZ_00266062"/>
        <obo:IAO_0000115>An archeological site. A ruined city of the Maya civilization in what is now the El Peten department of Guatemala.</obo:IAO_0000115>
        <oboInOwl:hasOBONamespace>GAZ</oboInOwl:hasOBONamespace>
        <oboInOwl:id>GAZ:00266067</oboInOwl:id>
        <rdfs:label>Machaquila</rdfs:label>
    </owl:NamedIndividual>
    


    <!-- http://purl.obolibrary.org/obo/GAZ_00266068 -->

    <owl:NamedIndividual rdf:about="http://purl.obolibrary.org/obo/GAZ_00266068">
        <obo:RO_0001025 rdf:resource="http://purl.obolibrary.org/obo/GAZ_00266062"/>
        <obo:IAO_0000115>An archeological site. An ancient city of the Maya civilization in the Peten Basin region of the central Maya lowlands.</obo:IAO_0000115>
        <oboInOwl:hasOBONamespace>GAZ</oboInOwl:hasOBONamespace>
        <oboInOwl:id>GAZ:00266068</oboInOwl:id>
        <rdfs:label>Naranjo</rdfs:label>
    </owl:NamedIndividual>
    


    <!-- http://purl.obolibrary.org/obo/GAZ_00266069 -->

    <owl:NamedIndividual rdf:about="http://purl.obolibrary.org/obo/GAZ_00266069">
        <obo:RO_0001025 rdf:resource="http://purl.obolibrary.org/obo/GAZ_00266062"/>
        <obo:IAO_0000115>A Mesoamerican archaeological site, and a former ceremonial center and city of the pre-Columbian Maya civilization. It is located in the northeastern portion of the Peten Basin region, in the modern-day Guatemalan department of Peten.</obo:IAO_0000115>
        <oboInOwl:hasOBONamespace>GAZ</oboInOwl:hasOBONamespace>
        <oboInOwl:id>GAZ:00266069</oboInOwl:id>
        <rdfs:label>Nakum</rdfs:label>
    </owl:NamedIndividual>
    


    <!-- http://purl.obolibrary.org/obo/GAZ_00266070 -->

    <owl:NamedIndividual rdf:about="http://purl.obolibrary.org/obo/GAZ_00266070">
        <obo:RO_0001025 rdf:resource="http://purl.obolibrary.org/obo/GAZ_00266062"/>
        <obo:IAO_0000115>An archeological site. A ruined city of the pre-Columbian Maya civilization located on the north bank of the Usumacinta River in the Peten department of Guatemala.</obo:IAO_0000115>
        <oboInOwl:hasOBONamespace>GAZ</oboInOwl:hasOBONamespace>
        <oboInOwl:id>GAZ:00266070</oboInOwl:id>
        <rdfs:label>Piedras Negras</rdfs:label>
    </owl:NamedIndividual>
    


    <!-- http://purl.obolibrary.org/obo/GAZ_00266071 -->

    <owl:NamedIndividual rdf:about="http://purl.obolibrary.org/obo/GAZ_00266071">
        <obo:RO_0001025 rdf:resource="http://purl.obolibrary.org/obo/GAZ_00266062"/>
        <obo:IAO_0000115>An archaeological site of the pre-Columbian Maya civilization, situated near the confluence of the Pasion and Salinas Rivers (where they combine to form the Usumacinta River), in the present-day department of Peten, Guatemala.</obo:IAO_0000115>
        <oboInOwl:hasOBONamespace>GAZ</oboInOwl:hasOBONamespace>
        <oboInOwl:id>GAZ:00266071</oboInOwl:id>
        <rdfs:label>Altar de Sacrificios</rdfs:label>
    </owl:NamedIndividual>
    


    <!-- http://purl.obolibrary.org/obo/GAZ_00266072 -->

    <owl:NamedIndividual rdf:about="http://purl.obolibrary.org/obo/GAZ_00266072">
        <obo:RO_0001025 rdf:resource="http://purl.obolibrary.org/obo/GAZ_00266062"/>
        <oboInOwl:hasOBONamespace>GAZ</oboInOwl:hasOBONamespace>
        <oboInOwl:id>GAZ:00266072</oboInOwl:id>
        <rdfs:label>Waka&apos;</rdfs:label>
    </owl:NamedIndividual>
    


    <!-- http://purl.obolibrary.org/obo/GAZ_00266073 -->

    <owl:NamedIndividual rdf:about="http://purl.obolibrary.org/obo/GAZ_00266073">
        <obo:RO_0001025 rdf:resource="http://purl.obolibrary.org/obo/GAZ_00266091"/>
        <obo:IAO_0000115>A Classic Period archaeological site of the Maya civilization located in the northern Peten Department of Guatemala.</obo:IAO_0000115>
        <oboInOwl:hasOBONamespace>GAZ</oboInOwl:hasOBONamespace>
        <oboInOwl:id>GAZ:00266073</oboInOwl:id>
        <rdfs:label>El Ceibal</rdfs:label>
    </owl:NamedIndividual>
    


    <!-- http://purl.obolibrary.org/obo/GAZ_00266074 -->

    <owl:NamedIndividual rdf:about="http://purl.obolibrary.org/obo/GAZ_00266074">
        <obo:RO_0001025 rdf:resource="http://purl.obolibrary.org/obo/GAZ_00248569"/>
        <obo:RO_0001025 rdf:resource="http://purl.obolibrary.org/obo/GAZ_00266062"/>
        <obo:IAO_0000115>A pre-Columbian Maya archaeological site in the Peten Basin in northern Guatemala. It occupies a group of small islands at the western end of Lake Yaxja.</obo:IAO_0000115>
        <oboInOwl:hasOBONamespace>GAZ</oboInOwl:hasOBONamespace>
        <oboInOwl:id>GAZ:00266074</oboInOwl:id>
        <rdfs:label>Topoxte</rdfs:label>
    </owl:NamedIndividual>
    


    <!-- http://purl.obolibrary.org/obo/GAZ_00266075 -->

    <owl:NamedIndividual rdf:about="http://purl.obolibrary.org/obo/GAZ_00266075">
        <obo:RO_0001025 rdf:resource="http://purl.obolibrary.org/obo/GAZ_00266062"/>
        <obo:IAO_0000115>A Mesoamerican archaeological site in the northeast of the Peten Basin region.</obo:IAO_0000115>
        <oboInOwl:hasOBONamespace>GAZ</oboInOwl:hasOBONamespace>
        <oboInOwl:id>GAZ:00266075</oboInOwl:id>
        <rdfs:label>Yaxha</rdfs:label>
    </owl:NamedIndividual>
    


    <!-- http://purl.obolibrary.org/obo/GAZ_00266076 -->

    <owl:NamedIndividual rdf:about="http://purl.obolibrary.org/obo/GAZ_00266076">
        <obo:RO_0001025 rdf:resource="http://purl.obolibrary.org/obo/GAZ_00266090"/>
        <obo:IAO_0000115>A Maya archeological site located in northern Guatemala&apos;s Petexbatun Basin, in the department of Peten.</obo:IAO_0000115>
        <oboInOwl:hasOBONamespace>GAZ</oboInOwl:hasOBONamespace>
        <oboInOwl:id>GAZ:00266076</oboInOwl:id>
        <rdfs:label>Aguateca</rdfs:label>
    </owl:NamedIndividual>
    


    <!-- http://purl.obolibrary.org/obo/GAZ_00266077 -->

    <owl:NamedIndividual rdf:about="http://purl.obolibrary.org/obo/GAZ_00266077">
        <obo:RO_0001025 rdf:resource="http://purl.obolibrary.org/obo/GAZ_00266062"/>
        <obo:IAO_0000115>An archaeological site of the pre-Columbian Maya civilization, located in the Pasion subregion of the central Maya lowlands in the present-day Guatemalan Department of El Peten.</obo:IAO_0000115>
        <oboInOwl:hasOBONamespace>GAZ</oboInOwl:hasOBONamespace>
        <oboInOwl:id>GAZ:00266077</oboInOwl:id>
        <rdfs:label>Cancuen</rdfs:label>
    </owl:NamedIndividual>
    


    <!-- http://purl.obolibrary.org/obo/GAZ_00266078 -->

    <owl:NamedIndividual rdf:about="http://purl.obolibrary.org/obo/GAZ_00266078">
        <obo:RO_0001025 rdf:resource="http://purl.obolibrary.org/obo/GAZ_00266062"/>
        <obo:IAO_0000115>A protected area. A World Heritage Site.</obo:IAO_0000115>
        <oboInOwl:hasOBONamespace>GAZ</oboInOwl:hasOBONamespace>
        <oboInOwl:id>GAZ:00266078</oboInOwl:id>
        <rdfs:label>Parque Nacional Tikal</rdfs:label>
    </owl:NamedIndividual>
    


    <!-- http://purl.obolibrary.org/obo/GAZ_00266079 -->

    <owl:NamedIndividual rdf:about="http://purl.obolibrary.org/obo/GAZ_00266079">
        <obo:RO_0001025 rdf:resource="http://purl.obolibrary.org/obo/GAZ_00068182"/>
        <obo:IAO_0000115>A pre-Columbian Maya archaeological site that dates to the Postclassic period. The site is located in the southern Maya lowlands on a small island in Lake Peten Itza.</obo:IAO_0000115>
        <oboInOwl:hasOBONamespace>GAZ</oboInOwl:hasOBONamespace>
        <oboInOwl:id>GAZ:00266079</oboInOwl:id>
        <rdfs:label>Tayasal</rdfs:label>
    </owl:NamedIndividual>
    


    <!-- http://purl.obolibrary.org/obo/GAZ_00266080 -->

    <owl:NamedIndividual rdf:about="http://purl.obolibrary.org/obo/GAZ_00266080">
        <obo:RO_0001025 rdf:resource="http://purl.obolibrary.org/obo/GAZ_00000508"/>
        <obo:IAO_0000115>A river.</obo:IAO_0000115>
        <oboInOwl:hasOBONamespace>GAZ</oboInOwl:hasOBONamespace>
        <oboInOwl:id>GAZ:00266080</oboInOwl:id>
        <rdfs:label>Rio San Pedro</rdfs:label>
    </owl:NamedIndividual>
    


    <!-- http://purl.obolibrary.org/obo/GAZ_00266081 -->

    <owl:NamedIndividual rdf:about="http://purl.obolibrary.org/obo/GAZ_00266081">
        <obo:RO_0001025 rdf:resource="http://purl.obolibrary.org/obo/GAZ_00266062"/>
        <obo:IAO_0000115>A Mesoamerican archaeological site of the pre-Columbian Maya civilization, located in the Peten Basin region around 20 km west of the major center of Tikal and approximately 26 km west of Uaxactun.</obo:IAO_0000115>
        <oboInOwl:hasOBONamespace>GAZ</oboInOwl:hasOBONamespace>
        <oboInOwl:id>GAZ:00266081</oboInOwl:id>
        <rdfs:label>El Zotz</rdfs:label>
    </owl:NamedIndividual>
    


    <!-- http://purl.obolibrary.org/obo/GAZ_00266082 -->

    <owl:NamedIndividual rdf:about="http://purl.obolibrary.org/obo/GAZ_00266082">
        <obo:RO_0001025 rdf:resource="http://purl.obolibrary.org/obo/GAZ_00266062"/>
        <obo:IAO_0000115>A Maya archaeological site that dates to the Classic and Postclassic Periods. It is located on the isthmus between the Peten Itza and Salpeten lakes, in the northern Peten Department of Guatemala.</obo:IAO_0000115>
        <oboInOwl:hasOBONamespace>GAZ</oboInOwl:hasOBONamespace>
        <oboInOwl:id>GAZ:00266082</oboInOwl:id>
        <rdfs:label>Ixlu</rdfs:label>
    </owl:NamedIndividual>
    


    <!-- http://purl.obolibrary.org/obo/GAZ_00266083 -->

    <owl:NamedIndividual rdf:about="http://purl.obolibrary.org/obo/GAZ_00266083">
        <obo:RO_0001025 rdf:resource="http://purl.obolibrary.org/obo/GAZ_00000509"/>
        <obo:IAO_0000115>A Pre-Columbian Maya archaeological site near Itzan, in the lower Pasion River region of the Peten Department of Guatemala.</obo:IAO_0000115>
        <oboInOwl:hasOBONamespace>GAZ</oboInOwl:hasOBONamespace>
        <oboInOwl:id>GAZ:00266083</oboInOwl:id>
        <rdfs:label>La Amelia</rdfs:label>
    </owl:NamedIndividual>
    


    <!-- http://purl.obolibrary.org/obo/GAZ_00266084 -->

    <owl:NamedIndividual rdf:about="http://purl.obolibrary.org/obo/GAZ_00266084">
        <obo:RO_0001025 rdf:resource="http://purl.obolibrary.org/obo/GAZ_00266060"/>
        <obo:IAO_0000115>A Maya archaeological site in the northern Peten region of Guatemala, located between the sites of El Mirador and El Tintal. It is located on a promontory 3.5 km south of the El Tigre complex of El Mirador, and it is considered a satellite of that city.</obo:IAO_0000115>
        <oboInOwl:hasOBONamespace>GAZ</oboInOwl:hasOBONamespace>
        <oboInOwl:id>GAZ:00266084</oboInOwl:id>
        <rdfs:label>La Muerta</rdfs:label>
    </owl:NamedIndividual>
    


    <!-- http://purl.obolibrary.org/obo/GAZ_00266085 -->

    <owl:NamedIndividual rdf:about="http://purl.obolibrary.org/obo/GAZ_00266085">
        <obo:RO_0001025 rdf:resource="http://purl.obolibrary.org/obo/GAZ_00266062"/>
        <obo:IAO_0000115>A Maya archeological site located just north of Lake Peten Itza in the Peten Basin region of the southern Maya lowlands. It is located a few kilometres from the modern village of San Jose, in Guatemala&apos;s northern department of Peten.</obo:IAO_0000115>
        <oboInOwl:hasOBONamespace>GAZ</oboInOwl:hasOBONamespace>
        <oboInOwl:id>GAZ:00266085</oboInOwl:id>
        <rdfs:label>Motul de San Jose</rdfs:label>
    </owl:NamedIndividual>
    


    <!-- http://purl.obolibrary.org/obo/GAZ_00266086 -->

    <owl:NamedIndividual rdf:about="http://purl.obolibrary.org/obo/GAZ_00266086">
        <obo:RO_0001025 rdf:resource="http://purl.obolibrary.org/obo/GAZ_00000508"/>
        <obo:IAO_0000115>A protected area.</obo:IAO_0000115>
        <oboInOwl:hasOBONamespace>GAZ</oboInOwl:hasOBONamespace>
        <oboInOwl:id>GAZ:00266086</oboInOwl:id>
        <rdfs:label>Parque Nacional Mirador - Rio Azul</rdfs:label>
    </owl:NamedIndividual>
    


    <!-- http://purl.obolibrary.org/obo/GAZ_00266087 -->

    <owl:NamedIndividual rdf:about="http://purl.obolibrary.org/obo/GAZ_00266087">
        <obo:RO_0001025 rdf:resource="http://purl.obolibrary.org/obo/GAZ_00000508"/>
        <obo:IAO_0000115>A protected area.</obo:IAO_0000115>
        <oboInOwl:hasOBONamespace>GAZ</oboInOwl:hasOBONamespace>
        <oboInOwl:id>GAZ:00266087</oboInOwl:id>
        <rdfs:label>Reserva Biologica San Roman</rdfs:label>
    </owl:NamedIndividual>
    


    <!-- http://purl.obolibrary.org/obo/GAZ_00266088 -->

    <owl:NamedIndividual rdf:about="http://purl.obolibrary.org/obo/GAZ_00266088">
        <obo:RO_0001025 rdf:resource="http://purl.obolibrary.org/obo/GAZ_00000508"/>
        <obo:IAO_0000115>A protected area.</obo:IAO_0000115>
        <oboInOwl:hasOBONamespace>GAZ</oboInOwl:hasOBONamespace>
        <oboInOwl:id>GAZ:00266088</oboInOwl:id>
        <rdfs:label>Monumento Natural Complejo II El Pucte</rdfs:label>
    </owl:NamedIndividual>
    


    <!-- http://purl.obolibrary.org/obo/GAZ_00266089 -->

    <owl:NamedIndividual rdf:about="http://purl.obolibrary.org/obo/GAZ_00266089">
        <obo:RO_0001025 rdf:resource="http://purl.obolibrary.org/obo/GAZ_00000508"/>
        <obo:IAO_0000115>A protected area.</obo:IAO_0000115>
        <oboInOwl:hasOBONamespace>GAZ</oboInOwl:hasOBONamespace>
        <oboInOwl:id>GAZ:00266089</oboInOwl:id>
        <rdfs:label>Reserva Forestal y Refugio de Vida Silvestre Petexbatun</rdfs:label>
    </owl:NamedIndividual>
    


    <!-- http://purl.obolibrary.org/obo/GAZ_00266090 -->

    <owl:NamedIndividual rdf:about="http://purl.obolibrary.org/obo/GAZ_00266090">
        <obo:RO_0001025 rdf:resource="http://purl.obolibrary.org/obo/GAZ_00266062"/>
        <obo:IAO_0000115>A protected area.</obo:IAO_0000115>
        <oboInOwl:hasOBONamespace>GAZ</oboInOwl:hasOBONamespace>
        <oboInOwl:id>GAZ:00266090</oboInOwl:id>
        <rdfs:label>Monumento Cultural y Parque Historico Aguateca</rdfs:label>
    </owl:NamedIndividual>
    


    <!-- http://purl.obolibrary.org/obo/GAZ_00266091 -->

    <owl:NamedIndividual rdf:about="http://purl.obolibrary.org/obo/GAZ_00266091">
        <obo:RO_0001025 rdf:resource="http://purl.obolibrary.org/obo/GAZ_00266062"/>
        <obo:IAO_0000115>A protected area.</obo:IAO_0000115>
        <oboInOwl:hasOBONamespace>GAZ</oboInOwl:hasOBONamespace>
        <oboInOwl:id>GAZ:00266091</oboInOwl:id>
        <rdfs:label>Monumento cultural El Ceibal</rdfs:label>
    </owl:NamedIndividual>
    


    <!-- http://purl.obolibrary.org/obo/GAZ_00266092 -->

    <owl:NamedIndividual rdf:about="http://purl.obolibrary.org/obo/GAZ_00266092">
        <obo:RO_0001025 rdf:resource="http://purl.obolibrary.org/obo/GAZ_00000508"/>
        <obo:IAO_0000115>A protected area.</obo:IAO_0000115>
        <oboInOwl:hasOBONamespace>GAZ</oboInOwl:hasOBONamespace>
        <oboInOwl:id>GAZ:00266092</oboInOwl:id>
        <rdfs:label>Reserva Biologica El Rosario</rdfs:label>
    </owl:NamedIndividual>
    


    <!-- http://purl.obolibrary.org/obo/GAZ_00266093 -->

    <owl:NamedIndividual rdf:about="http://purl.obolibrary.org/obo/GAZ_00266093">
        <obo:RO_0001025 rdf:resource="http://purl.obolibrary.org/obo/GAZ_00000508"/>
        <obo:IAO_0000115>A protected area.</obo:IAO_0000115>
        <oboInOwl:hasOBONamespace>GAZ</oboInOwl:hasOBONamespace>
        <oboInOwl:id>GAZ:00266093</oboInOwl:id>
        <rdfs:label>Reserva Natural Privada La Cumbre Flor de la Paz</rdfs:label>
    </owl:NamedIndividual>
    


    <!-- http://purl.obolibrary.org/obo/GAZ_00266094 -->

    <owl:NamedIndividual rdf:about="http://purl.obolibrary.org/obo/GAZ_00266094">
        <obo:RO_0001025 rdf:resource="http://purl.obolibrary.org/obo/GAZ_00000508"/>
        <obo:IAO_0000115>A protected area.</obo:IAO_0000115>
        <oboInOwl:hasOBONamespace>GAZ</oboInOwl:hasOBONamespace>
        <oboInOwl:id>GAZ:00266094</oboInOwl:id>
        <rdfs:label>Reserva Natural Privada Dona Chanita, Flor de la Paz</rdfs:label>
    </owl:NamedIndividual>
    


    <!-- http://purl.obolibrary.org/obo/GAZ_00266095 -->

    <owl:NamedIndividual rdf:about="http://purl.obolibrary.org/obo/GAZ_00266095">
        <obo:RO_0001025 rdf:resource="http://purl.obolibrary.org/obo/GAZ_00000508"/>
        <obo:IAO_0000115>A protected area.</obo:IAO_0000115>
        <oboInOwl:hasOBONamespace>GAZ</oboInOwl:hasOBONamespace>
        <oboInOwl:id>GAZ:00266095</oboInOwl:id>
        <rdfs:label>Reserva Natural Privada Ceibo Mocho, Flor de la Paz</rdfs:label>
    </owl:NamedIndividual>
    


    <!-- http://purl.obolibrary.org/obo/GAZ_00266096 -->

    <owl:NamedIndividual rdf:about="http://purl.obolibrary.org/obo/GAZ_00266096">
        <obo:RO_0001025 rdf:resource="http://purl.obolibrary.org/obo/GAZ_00068175"/>
        <obo:IAO_0000115>A lake.</obo:IAO_0000115>
        <oboInOwl:hasOBONamespace>GAZ</oboInOwl:hasOBONamespace>
        <oboInOwl:id>GAZ:00266096</oboInOwl:id>
        <rdfs:label>Laguna San Diego</rdfs:label>
    </owl:NamedIndividual>
    


    <!-- http://purl.obolibrary.org/obo/GAZ_00266097 -->

    <owl:NamedIndividual rdf:about="http://purl.obolibrary.org/obo/GAZ_00266097">
        <obo:RO_0001025 rdf:resource="http://purl.obolibrary.org/obo/GAZ_00068174"/>
        <obo:IAO_0000115>A biosphere reserve in the north of Guatemala. It is located in the municipalities of San Luis, Poptun, Dolores, and Melchor de Mencos in the department of El Peten.</obo:IAO_0000115>
        <oboInOwl:hasOBONamespace>GAZ</oboInOwl:hasOBONamespace>
        <oboInOwl:id>GAZ:00266097</oboInOwl:id>
        <rdfs:label>La Reserva de Biosfera Complejo Chiquibul/Montana</rdfs:label>
    </owl:NamedIndividual>
    


    <!-- http://purl.obolibrary.org/obo/GAZ_00266098 -->

    <owl:NamedIndividual rdf:about="http://purl.obolibrary.org/obo/GAZ_00266098">
        <obo:RO_0001025 rdf:resource="http://purl.obolibrary.org/obo/GAZ_00000508"/>
        <obo:IAO_0000115>A protected area.</obo:IAO_0000115>
        <oboInOwl:hasOBONamespace>GAZ</oboInOwl:hasOBONamespace>
        <oboInOwl:id>GAZ:00266098</oboInOwl:id>
        <rdfs:label>Reserva Forestal Xutilja</rdfs:label>
    </owl:NamedIndividual>
    


    <!-- http://purl.obolibrary.org/obo/GAZ_00266099 -->

    <owl:NamedIndividual rdf:about="http://purl.obolibrary.org/obo/GAZ_00266099">
        <obo:RO_0001025 rdf:resource="http://purl.obolibrary.org/obo/GAZ_00000508"/>
        <obo:IAO_0000115>A protected area.</obo:IAO_0000115>
        <oboInOwl:hasOBONamespace>GAZ</oboInOwl:hasOBONamespace>
        <oboInOwl:id>GAZ:00266099</oboInOwl:id>
        <rdfs:label>Reserva Forestal Machaquila</rdfs:label>
    </owl:NamedIndividual>
    


    <!-- http://purl.obolibrary.org/obo/GAZ_00266100 -->

    <owl:NamedIndividual rdf:about="http://purl.obolibrary.org/obo/GAZ_00266100">
        <obo:RO_0001025 rdf:resource="http://purl.obolibrary.org/obo/GAZ_00000508"/>
        <obo:IAO_0000115>A protected area.</obo:IAO_0000115>
        <oboInOwl:hasOBONamespace>GAZ</oboInOwl:hasOBONamespace>
        <oboInOwl:id>GAZ:00266100</oboInOwl:id>
        <rdfs:label>Reserva de Biosfera Complejo III Montanas</rdfs:label>
    </owl:NamedIndividual>
    


    <!-- http://purl.obolibrary.org/obo/GAZ_00266101 -->

    <owl:NamedIndividual rdf:about="http://purl.obolibrary.org/obo/GAZ_00266101">
        <obo:RO_0001025 rdf:resource="http://purl.obolibrary.org/obo/GAZ_00000508"/>
        <obo:IAO_0000115>A protected area.</obo:IAO_0000115>
        <oboInOwl:hasOBONamespace>GAZ</oboInOwl:hasOBONamespace>
        <oboInOwl:id>GAZ:00266101</oboInOwl:id>
        <rdfs:label>Monumento Natural que rodea La Laguna del Tigre</rdfs:label>
    </owl:NamedIndividual>
    


    <!-- http://purl.obolibrary.org/obo/GAZ_00266102 -->

    <owl:NamedIndividual rdf:about="http://purl.obolibrary.org/obo/GAZ_00266102">
        <obo:RO_0001025 rdf:resource="http://purl.obolibrary.org/obo/GAZ_00000508"/>
        <obo:IAO_0000115>A protected area.</obo:IAO_0000115>
        <oboInOwl:hasOBONamespace>GAZ</oboInOwl:hasOBONamespace>
        <oboInOwl:id>GAZ:00266102</oboInOwl:id>
        <rdfs:label>Reserva Biologica Sierra del Lacandon</rdfs:label>
    </owl:NamedIndividual>
    


    <!-- http://purl.obolibrary.org/obo/GAZ_00266103 -->

    <owl:NamedIndividual rdf:about="http://purl.obolibrary.org/obo/GAZ_00266103">
        <obo:RO_0001025 rdf:resource="http://purl.obolibrary.org/obo/GAZ_00000508"/>
        <obo:IAO_0000115>A protected area.</obo:IAO_0000115>
        <oboInOwl:hasOBONamespace>GAZ</oboInOwl:hasOBONamespace>
        <oboInOwl:id>GAZ:00266103</oboInOwl:id>
        <rdfs:label>Biotopo Protegido Cerro Cahui</rdfs:label>
    </owl:NamedIndividual>
    


    <!-- http://purl.obolibrary.org/obo/GAZ_00266104 -->

    <owl:NamedIndividual rdf:about="http://purl.obolibrary.org/obo/GAZ_00266104">
        <obo:RO_0001025 rdf:resource="http://purl.obolibrary.org/obo/GAZ_00068174"/>
        <obo:IAO_0000115>A lake.</obo:IAO_0000115>
        <oboInOwl:hasOBONamespace>GAZ</oboInOwl:hasOBONamespace>
        <oboInOwl:id>GAZ:00266104</oboInOwl:id>
        <rdfs:label>Laguna Colorado</rdfs:label>
    </owl:NamedIndividual>
    


    <!-- http://purl.obolibrary.org/obo/GAZ_00266105 -->

    <owl:NamedIndividual rdf:about="http://purl.obolibrary.org/obo/GAZ_00266105">
        <obo:RO_0001025 rdf:resource="http://purl.obolibrary.org/obo/GAZ_00068174"/>
        <obo:IAO_0000115>A lake.</obo:IAO_0000115>
        <oboInOwl:hasOBONamespace>GAZ</oboInOwl:hasOBONamespace>
        <oboInOwl:id>GAZ:00266105</oboInOwl:id>
        <rdfs:label>Laguna del Julek</rdfs:label>
    </owl:NamedIndividual>
    


    <!-- http://purl.obolibrary.org/obo/GAZ_00266106 -->

    <owl:NamedIndividual rdf:about="http://purl.obolibrary.org/obo/GAZ_00266106">
        <obo:RO_0001025 rdf:resource="http://purl.obolibrary.org/obo/GAZ_00068174"/>
        <obo:IAO_0000115>A lake.</obo:IAO_0000115>
        <oboInOwl:hasOBONamespace>GAZ</oboInOwl:hasOBONamespace>
        <oboInOwl:id>GAZ:00266106</oboInOwl:id>
        <rdfs:label>Laguna Blanca</rdfs:label>
    </owl:NamedIndividual>
    


    <!-- http://purl.obolibrary.org/obo/GAZ_00266107 -->

    <owl:NamedIndividual rdf:about="http://purl.obolibrary.org/obo/GAZ_00266107">
        <obo:RO_0001025 rdf:resource="http://purl.obolibrary.org/obo/GAZ_00068174"/>
        <obo:IAO_0000115>A lake.</obo:IAO_0000115>
        <oboInOwl:hasOBONamespace>GAZ</oboInOwl:hasOBONamespace>
        <oboInOwl:id>GAZ:00266107</oboInOwl:id>
        <rdfs:label>Laguna el Ocote</rdfs:label>
    </owl:NamedIndividual>
    


    <!-- http://purl.obolibrary.org/obo/GAZ_00266108 -->

    <owl:NamedIndividual rdf:about="http://purl.obolibrary.org/obo/GAZ_00266108">
        <obo:RO_0001025 rdf:resource="http://purl.obolibrary.org/obo/GAZ_00068174"/>
        <obo:IAO_0000115>A lake.</obo:IAO_0000115>
        <oboInOwl:hasOBONamespace>GAZ</oboInOwl:hasOBONamespace>
        <oboInOwl:id>GAZ:00266108</oboInOwl:id>
        <rdfs:label>Laguna los lagartos</rdfs:label>
    </owl:NamedIndividual>
    


    <!-- http://purl.obolibrary.org/obo/GAZ_00266109 -->

    <owl:NamedIndividual rdf:about="http://purl.obolibrary.org/obo/GAZ_00266109">
        <obo:RO_0001025 rdf:resource="http://purl.obolibrary.org/obo/GAZ_00068175"/>
        <obo:IAO_0000115>A lake.</obo:IAO_0000115>
        <oboInOwl:hasOBONamespace>GAZ</oboInOwl:hasOBONamespace>
        <oboInOwl:id>GAZ:00266109</oboInOwl:id>
        <rdfs:label>Laguna La Gloria</rdfs:label>
    </owl:NamedIndividual>
    


    <!-- http://purl.obolibrary.org/obo/GAZ_00266110 -->

    <owl:NamedIndividual rdf:about="http://purl.obolibrary.org/obo/GAZ_00266110">
        <obo:RO_0001025 rdf:resource="http://purl.obolibrary.org/obo/GAZ_00068175"/>
        <obo:IAO_0000115>A lake.</obo:IAO_0000115>
        <oboInOwl:hasOBONamespace>GAZ</oboInOwl:hasOBONamespace>
        <oboInOwl:id>GAZ:00266110</oboInOwl:id>
        <rdfs:label>Laguna Larga</rdfs:label>
    </owl:NamedIndividual>
    


    <!-- http://purl.obolibrary.org/obo/GAZ_00266111 -->

    <owl:NamedIndividual rdf:about="http://purl.obolibrary.org/obo/GAZ_00266111">
        <obo:RO_0001025 rdf:resource="http://purl.obolibrary.org/obo/GAZ_00068175"/>
        <obo:IAO_0000115>A lake.</obo:IAO_0000115>
        <oboInOwl:hasOBONamespace>GAZ</oboInOwl:hasOBONamespace>
        <oboInOwl:id>GAZ:00266111</oboInOwl:id>
        <rdfs:label>Laguna Mendoza</rdfs:label>
    </owl:NamedIndividual>
    


    <!-- http://purl.obolibrary.org/obo/GAZ_00266112 -->

    <owl:NamedIndividual rdf:about="http://purl.obolibrary.org/obo/GAZ_00266112">
        <obo:RO_0001025 rdf:resource="http://purl.obolibrary.org/obo/GAZ_00068175"/>
        <obo:IAO_0000115>A lake.</obo:IAO_0000115>
        <oboInOwl:hasOBONamespace>GAZ</oboInOwl:hasOBONamespace>
        <oboInOwl:id>GAZ:00266112</oboInOwl:id>
        <rdfs:label>Laguna Pucte</rdfs:label>
    </owl:NamedIndividual>
    


    <!-- http://purl.obolibrary.org/obo/GAZ_00266113 -->

    <owl:NamedIndividual rdf:about="http://purl.obolibrary.org/obo/GAZ_00266113">
        <obo:RO_0001025 rdf:resource="http://purl.obolibrary.org/obo/GAZ_00068175"/>
        <obo:IAO_0000115>A lake.</obo:IAO_0000115>
        <oboInOwl:hasOBONamespace>GAZ</oboInOwl:hasOBONamespace>
        <oboInOwl:id>GAZ:00266113</oboInOwl:id>
        <rdfs:label>Laguna Yaxtunila</rdfs:label>
    </owl:NamedIndividual>
    


    <!-- http://purl.obolibrary.org/obo/GAZ_00266114 -->

    <owl:NamedIndividual rdf:about="http://purl.obolibrary.org/obo/GAZ_00266114">
        <obo:RO_0001025 rdf:resource="http://purl.obolibrary.org/obo/GAZ_00068175"/>
        <obo:IAO_0000115>A lake.</obo:IAO_0000115>
        <oboInOwl:hasOBONamespace>GAZ</oboInOwl:hasOBONamespace>
        <oboInOwl:id>GAZ:00266114</oboInOwl:id>
        <rdfs:label>Laguna El Repasto</rdfs:label>
    </owl:NamedIndividual>
    


    <!-- http://purl.obolibrary.org/obo/GAZ_00266115 -->

    <owl:NamedIndividual rdf:about="http://purl.obolibrary.org/obo/GAZ_00266115">
        <obo:RO_0001025 rdf:resource="http://purl.obolibrary.org/obo/GAZ_00068175"/>
        <obo:IAO_0000115>A lake.</obo:IAO_0000115>
        <oboInOwl:hasOBONamespace>GAZ</oboInOwl:hasOBONamespace>
        <oboInOwl:id>GAZ:00266115</oboInOwl:id>
        <rdfs:label>Laguna El Reloj</rdfs:label>
    </owl:NamedIndividual>
    


    <!-- http://purl.obolibrary.org/obo/GAZ_00266116 -->

    <owl:NamedIndividual rdf:about="http://purl.obolibrary.org/obo/GAZ_00266116">
        <obo:RO_0001025 rdf:resource="http://purl.obolibrary.org/obo/GAZ_00068175"/>
        <obo:IAO_0000115>A lake.</obo:IAO_0000115>
        <oboInOwl:hasOBONamespace>GAZ</oboInOwl:hasOBONamespace>
        <oboInOwl:id>GAZ:00266116</oboInOwl:id>
        <rdfs:label>Laguna Las Cuaches</rdfs:label>
    </owl:NamedIndividual>
    


    <!-- http://purl.obolibrary.org/obo/GAZ_00266117 -->

    <owl:NamedIndividual rdf:about="http://purl.obolibrary.org/obo/GAZ_00266117">
        <obo:RO_0001025 rdf:resource="http://purl.obolibrary.org/obo/GAZ_00068175"/>
        <obo:IAO_0000115>A lake.</obo:IAO_0000115>
        <oboInOwl:hasOBONamespace>GAZ</oboInOwl:hasOBONamespace>
        <oboInOwl:id>GAZ:00266117</oboInOwl:id>
        <rdfs:label>Laguna Agua Dulce</rdfs:label>
    </owl:NamedIndividual>
    


    <!-- http://purl.obolibrary.org/obo/GAZ_00266118 -->

    <owl:NamedIndividual rdf:about="http://purl.obolibrary.org/obo/GAZ_00266118">
        <obo:RO_0001025 rdf:resource="http://purl.obolibrary.org/obo/GAZ_00068175"/>
        <obo:IAO_0000115>A lake.</obo:IAO_0000115>
        <oboInOwl:hasOBONamespace>GAZ</oboInOwl:hasOBONamespace>
        <oboInOwl:id>GAZ:00266118</oboInOwl:id>
        <rdfs:label>Laguna Bolamchac</rdfs:label>
    </owl:NamedIndividual>
    


    <!-- http://purl.obolibrary.org/obo/GAZ_00266119 -->

    <owl:NamedIndividual rdf:about="http://purl.obolibrary.org/obo/GAZ_00266119">
        <obo:RO_0001025 rdf:resource="http://purl.obolibrary.org/obo/GAZ_00068175"/>
        <obo:IAO_0000115>A lake.</obo:IAO_0000115>
        <oboInOwl:hasOBONamespace>GAZ</oboInOwl:hasOBONamespace>
        <oboInOwl:id>GAZ:00266119</oboInOwl:id>
        <rdfs:label>Laguna Bucutal</rdfs:label>
    </owl:NamedIndividual>
    


    <!-- http://purl.obolibrary.org/obo/GAZ_00266120 -->

    <owl:NamedIndividual rdf:about="http://purl.obolibrary.org/obo/GAZ_00266120">
        <obo:RO_0001025 rdf:resource="http://purl.obolibrary.org/obo/GAZ_00068175"/>
        <obo:IAO_0000115>A lake.</obo:IAO_0000115>
        <oboInOwl:hasOBONamespace>GAZ</oboInOwl:hasOBONamespace>
        <oboInOwl:id>GAZ:00266120</oboInOwl:id>
        <rdfs:label>Laguna Buena Vista</rdfs:label>
    </owl:NamedIndividual>
    


    <!-- http://purl.obolibrary.org/obo/GAZ_00266121 -->

    <owl:NamedIndividual rdf:about="http://purl.obolibrary.org/obo/GAZ_00266121">
        <obo:RO_0001025 rdf:resource="http://purl.obolibrary.org/obo/GAZ_00068175"/>
        <obo:IAO_0000115>A lake.</obo:IAO_0000115>
        <oboInOwl:hasOBONamespace>GAZ</oboInOwl:hasOBONamespace>
        <oboInOwl:id>GAZ:00266121</oboInOwl:id>
        <rdfs:label>Laguna El Curro</rdfs:label>
    </owl:NamedIndividual>
    


    <!-- http://purl.obolibrary.org/obo/GAZ_00266122 -->

    <owl:NamedIndividual rdf:about="http://purl.obolibrary.org/obo/GAZ_00266122">
        <obo:RO_0001025 rdf:resource="http://purl.obolibrary.org/obo/GAZ_00068175"/>
        <obo:IAO_0000115>A lake.</obo:IAO_0000115>
        <oboInOwl:hasOBONamespace>GAZ</oboInOwl:hasOBONamespace>
        <oboInOwl:id>GAZ:00266122</oboInOwl:id>
        <rdfs:label>Laguna Itzan</rdfs:label>
    </owl:NamedIndividual>
    


    <!-- http://purl.obolibrary.org/obo/GAZ_00266123 -->

    <owl:NamedIndividual rdf:about="http://purl.obolibrary.org/obo/GAZ_00266123">
        <obo:RO_0001025 rdf:resource="http://purl.obolibrary.org/obo/GAZ_00068175"/>
        <obo:IAO_0000115>A lake.</obo:IAO_0000115>
        <oboInOwl:hasOBONamespace>GAZ</oboInOwl:hasOBONamespace>
        <oboInOwl:id>GAZ:00266123</oboInOwl:id>
        <rdfs:label>Laguna Lacandon</rdfs:label>
    </owl:NamedIndividual>
    


    <!-- http://purl.obolibrary.org/obo/GAZ_00266125 -->

    <owl:NamedIndividual rdf:about="http://purl.obolibrary.org/obo/GAZ_00266125">
        <obo:RO_0001025 rdf:resource="http://purl.obolibrary.org/obo/GAZ_00000508"/>
        <obo:IAO_0000115>A river located in the northern lowlands region of Guatemala.</obo:IAO_0000115>
        <oboInOwl:hasOBONamespace>GAZ</oboInOwl:hasOBONamespace>
        <oboInOwl:id>GAZ:00266125</oboInOwl:id>
        <rdfs:label>Rio la Pasion</rdfs:label>
    </owl:NamedIndividual>
    


    <!-- http://purl.obolibrary.org/obo/GAZ_00266126 -->

    <owl:NamedIndividual rdf:about="http://purl.obolibrary.org/obo/GAZ_00266126">
        <obo:RO_0001025 rdf:resource="http://purl.obolibrary.org/obo/GAZ_00000508"/>
        <obo:IAO_0000115>A river.</obo:IAO_0000115>
        <oboInOwl:hasOBONamespace>GAZ</oboInOwl:hasOBONamespace>
        <oboInOwl:id>GAZ:00266126</oboInOwl:id>
        <rdfs:label>Rio San Juan</rdfs:label>
    </owl:NamedIndividual>
    


    <!-- http://purl.obolibrary.org/obo/GAZ_00266127 -->

    <owl:NamedIndividual rdf:about="http://purl.obolibrary.org/obo/GAZ_00266127">
        <obo:RO_0001025 rdf:resource="http://purl.obolibrary.org/obo/GAZ_00000508"/>
        <obo:IAO_0000115>A river.</obo:IAO_0000115>
        <oboInOwl:hasOBONamespace>GAZ</oboInOwl:hasOBONamespace>
        <oboInOwl:id>GAZ:00266127</oboInOwl:id>
        <rdfs:label>Rio Machaquila</rdfs:label>
    </owl:NamedIndividual>
    


    <!-- http://purl.obolibrary.org/obo/GAZ_00266128 -->

    <owl:NamedIndividual rdf:about="http://purl.obolibrary.org/obo/GAZ_00266128">
        <obo:RO_0001025 rdf:resource="http://purl.obolibrary.org/obo/GAZ_00000508"/>
        <obo:IAO_0000115>A river.</obo:IAO_0000115>
        <oboInOwl:hasOBONamespace>GAZ</oboInOwl:hasOBONamespace>
        <oboInOwl:id>GAZ:00266128</oboInOwl:id>
        <rdfs:label>Rio Cancuen</rdfs:label>
    </owl:NamedIndividual>
    


    <!-- http://purl.obolibrary.org/obo/GAZ_00266130 -->

    <owl:NamedIndividual rdf:about="http://purl.obolibrary.org/obo/GAZ_00266130">
        <obo:IAO_0000115>A reinforced concrete dam and power plant spanning the Chixoy River between the Departments of Baja Verapaz, El Quiche and Alta Verapaz, Guatemala. Constructed 1976-1983.</obo:IAO_0000115>
        <oboInOwl:hasOBONamespace>GAZ</oboInOwl:hasOBONamespace>
        <oboInOwl:id>GAZ:00266130</oboInOwl:id>
        <rdfs:label>Planta Hidroelectrica Chixoy</rdfs:label>
    </owl:NamedIndividual>
    


    <!-- http://purl.obolibrary.org/obo/GAZ_00266133 -->

    <owl:NamedIndividual rdf:about="http://purl.obolibrary.org/obo/GAZ_00266133">
        <obo:RO_0001025 rdf:resource="http://purl.obolibrary.org/obo/GAZ_00000509"/>
        <obo:IAO_0000115>A protected area. Located in El Peten, Guatemala, on the eastern edge of the town of Sayaxche.</obo:IAO_0000115>
        <oboInOwl:hasOBONamespace>GAZ</oboInOwl:hasOBONamespace>
        <oboInOwl:id>GAZ:00266133</oboInOwl:id>
        <rdfs:label>Parque Nacional El Rosario</rdfs:label>
    </owl:NamedIndividual>
    


    <!-- http://purl.obolibrary.org/obo/GAZ_00266134 -->

    <owl:NamedIndividual rdf:about="http://purl.obolibrary.org/obo/GAZ_00266134">
        <obo:RO_0001025 rdf:resource="http://purl.obolibrary.org/obo/GAZ_00266133"/>
        <obo:IAO_0000115>A lake.</obo:IAO_0000115>
        <oboInOwl:hasOBONamespace>GAZ</oboInOwl:hasOBONamespace>
        <oboInOwl:id>GAZ:00266134</oboInOwl:id>
        <rdfs:label>Laguna El Rosario</rdfs:label>
    </owl:NamedIndividual>
    


    <!-- http://purl.obolibrary.org/obo/GAZ_00266135 -->

    <owl:NamedIndividual rdf:about="http://purl.obolibrary.org/obo/GAZ_00266135">
        <obo:RO_0001025 rdf:resource="http://purl.obolibrary.org/obo/GAZ_00068184"/>
        <obo:IAO_0000115>A stratovolcano in Guatemala.</obo:IAO_0000115>
        <oboInOwl:hasOBONamespace>GAZ</oboInOwl:hasOBONamespace>
        <oboInOwl:id>GAZ:00266135</oboInOwl:id>
        <rdfs:label>Volcan Siete Orejas</rdfs:label>
    </owl:NamedIndividual>
    


    <!-- http://purl.obolibrary.org/obo/GAZ_00266136 -->

    <owl:NamedIndividual rdf:about="http://purl.obolibrary.org/obo/GAZ_00266136">
        <obo:RO_0001025 rdf:resource="http://purl.obolibrary.org/obo/GAZ_00068222"/>
        <obo:IAO_0000115>An archeological site in the southwest of the El Quiche department of Guatemala.</obo:IAO_0000115>
        <oboInOwl:hasOBONamespace>GAZ</oboInOwl:hasOBONamespace>
        <oboInOwl:id>GAZ:00266136</oboInOwl:id>
        <rdfs:label>Q&apos;umarkaj</rdfs:label>
    </owl:NamedIndividual>
    


    <!-- http://purl.obolibrary.org/obo/GAZ_00266137 -->

    <owl:NamedIndividual rdf:about="http://purl.obolibrary.org/obo/GAZ_00266137">
        <obo:RO_0001025 rdf:resource="http://purl.obolibrary.org/obo/GAZ_00000520"/>
        <obo:IAO_0000115>An archeological site of the Maya civilization in the highlands of Guatemala.</obo:IAO_0000115>
        <oboInOwl:hasOBONamespace>GAZ</oboInOwl:hasOBONamespace>
        <oboInOwl:id>GAZ:00266137</oboInOwl:id>
        <rdfs:label>Chitinamit</rdfs:label>
    </owl:NamedIndividual>
    


    <!-- http://purl.obolibrary.org/obo/GAZ_00266138 -->

    <owl:NamedIndividual rdf:about="http://purl.obolibrary.org/obo/GAZ_00266138">
        <obo:RO_0001025 rdf:resource="http://purl.obolibrary.org/obo/GAZ_00068218"/>
        <obo:IAO_0000115>A lake.</obo:IAO_0000115>
        <oboInOwl:hasOBONamespace>GAZ</oboInOwl:hasOBONamespace>
        <oboInOwl:id>GAZ:00266138</oboInOwl:id>
        <rdfs:label>Laguna de San Antonio</rdfs:label>
    </owl:NamedIndividual>
    


    <!-- http://purl.obolibrary.org/obo/GAZ_00266139 -->

    <owl:NamedIndividual rdf:about="http://purl.obolibrary.org/obo/GAZ_00266139">
        <obo:RO_0001025 rdf:resource="http://purl.obolibrary.org/obo/GAZ_00068222"/>
        <obo:IAO_0000115>A lake.</obo:IAO_0000115>
        <oboInOwl:hasOBONamespace>GAZ</oboInOwl:hasOBONamespace>
        <oboInOwl:id>GAZ:00266139</oboInOwl:id>
        <rdfs:label>Laguna de Lemoa</rdfs:label>
    </owl:NamedIndividual>
    


    <!-- http://purl.obolibrary.org/obo/GAZ_00266140 -->

    <owl:NamedIndividual rdf:about="http://purl.obolibrary.org/obo/GAZ_00266140">
        <obo:RO_0001025 rdf:resource="http://purl.obolibrary.org/obo/GAZ_00068222"/>
        <obo:IAO_0000115>A lake.</obo:IAO_0000115>
        <oboInOwl:hasOBONamespace>GAZ</oboInOwl:hasOBONamespace>
        <oboInOwl:id>GAZ:00266140</oboInOwl:id>
        <rdfs:label>Laguna de La Estancia</rdfs:label>
    </owl:NamedIndividual>
    


    <!-- http://purl.obolibrary.org/obo/GAZ_00266141 -->

    <owl:NamedIndividual rdf:about="http://purl.obolibrary.org/obo/GAZ_00266141">
        <obo:RO_0001025 rdf:resource="http://purl.obolibrary.org/obo/GAZ_00000517"/>
        <obo:IAO_0000115>A protected area in the department of El Quiche.</obo:IAO_0000115>
        <oboInOwl:hasOBONamespace>GAZ</oboInOwl:hasOBONamespace>
        <oboInOwl:id>GAZ:00266141</oboInOwl:id>
        <rdfs:label>Biosfera Ixil</rdfs:label>
    </owl:NamedIndividual>
    


    <!-- http://purl.obolibrary.org/obo/GAZ_00266142 -->

    <owl:NamedIndividual rdf:about="http://purl.obolibrary.org/obo/GAZ_00266142">
        <obo:RO_0001025 rdf:resource="http://purl.obolibrary.org/obo/GAZ_00000519"/>
        <obo:IAO_0000115>An archaeological site of the pre-Columbian Maya civilization, located in the western Guatemala highlands.</obo:IAO_0000115>
        <oboInOwl:hasOBONamespace>GAZ</oboInOwl:hasOBONamespace>
        <oboInOwl:id>GAZ:00266142</oboInOwl:id>
        <rdfs:label>Nebaj</rdfs:label>
    </owl:NamedIndividual>
    


    <!-- http://purl.obolibrary.org/obo/GAZ_00266152 -->

    <owl:NamedIndividual rdf:about="http://purl.obolibrary.org/obo/GAZ_00266152">
        <obo:RO_0001025 rdf:resource="http://purl.obolibrary.org/obo/GAZ_00000483"/>
        <obo:IAO_0000115>A river.</obo:IAO_0000115>
        <oboInOwl:hasOBONamespace>GAZ</oboInOwl:hasOBONamespace>
        <oboInOwl:id>GAZ:00266152</oboInOwl:id>
        <rdfs:label>Rio Apal</rdfs:label>
    </owl:NamedIndividual>
    


    <!-- http://purl.obolibrary.org/obo/GAZ_00266153 -->

    <owl:NamedIndividual rdf:about="http://purl.obolibrary.org/obo/GAZ_00266153">
        <obo:RO_0001025 rdf:resource="http://purl.obolibrary.org/obo/GAZ_00000483"/>
        <obo:IAO_0000115>A river.</obo:IAO_0000115>
        <oboInOwl:hasOBONamespace>GAZ</oboInOwl:hasOBONamespace>
        <oboInOwl:id>GAZ:00266153</oboInOwl:id>
        <rdfs:label>Ruio Chom</rdfs:label>
    </owl:NamedIndividual>
    


    <!-- http://purl.obolibrary.org/obo/GAZ_00266154 -->

    <owl:NamedIndividual rdf:about="http://purl.obolibrary.org/obo/GAZ_00266154">
        <obo:RO_0001025 rdf:resource="http://purl.obolibrary.org/obo/GAZ_00000483"/>
        <obo:IAO_0000115>A river.</obo:IAO_0000115>
        <oboInOwl:hasOBONamespace>GAZ</oboInOwl:hasOBONamespace>
        <oboInOwl:id>GAZ:00266154</oboInOwl:id>
        <rdfs:label>Rio Coxton</rdfs:label>
    </owl:NamedIndividual>
    


    <!-- http://purl.obolibrary.org/obo/GAZ_00266163 -->

    <owl:NamedIndividual rdf:about="http://purl.obolibrary.org/obo/GAZ_00266163">
        <obo:RO_0001025 rdf:resource="http://purl.obolibrary.org/obo/GAZ_00000522"/>
        <obo:IAO_0000115>The largest preclassic archeological site to be discovered on Guatemalan Pacific coast.</obo:IAO_0000115>
        <oboInOwl:hasOBONamespace>GAZ</oboInOwl:hasOBONamespace>
        <oboInOwl:id>GAZ:00266163</oboInOwl:id>
        <rdfs:label>Ujuxte</rdfs:label>
    </owl:NamedIndividual>
    


    <!-- http://purl.obolibrary.org/obo/GAZ_00266164 -->

    <owl:NamedIndividual rdf:about="http://purl.obolibrary.org/obo/GAZ_00266164">
        <obo:RO_0001025 rdf:resource="http://purl.obolibrary.org/obo/GAZ_00000523"/>
        <obo:IAO_0000115>A pre-Columbian archaeological site in Guatemala.</obo:IAO_0000115>
        <oboInOwl:hasOBONamespace>GAZ</oboInOwl:hasOBONamespace>
        <oboInOwl:id>GAZ:00266164</oboInOwl:id>
        <rdfs:label>Takalik Abaj</rdfs:label>
    </owl:NamedIndividual>
    


    <!-- http://purl.obolibrary.org/obo/GAZ_00266165 -->

    <owl:NamedIndividual rdf:about="http://purl.obolibrary.org/obo/GAZ_00266165">
        <obo:RO_0001025 rdf:resource="http://purl.obolibrary.org/obo/GAZ_00000522"/>
        <obo:IAO_0000115>A river in Guatemala flowing from the Guatemalan highlands into the Pacific Ocean. It passes through the Department of Retalhuleu.</obo:IAO_0000115>
        <oboInOwl:hasOBONamespace>GAZ</oboInOwl:hasOBONamespace>
        <oboInOwl:id>GAZ:00266165</oboInOwl:id>
        <rdfs:label>Rio Ixchaya</rdfs:label>
    </owl:NamedIndividual>
    


    <!-- http://purl.obolibrary.org/obo/GAZ_00266166 -->

    <owl:NamedIndividual rdf:about="http://purl.obolibrary.org/obo/GAZ_00266166">
        <obo:RO_0001025 rdf:resource="http://purl.obolibrary.org/obo/GAZ_00000529"/>
        <obo:IAO_0000115>A protected area.</obo:IAO_0000115>
        <oboInOwl:hasOBONamespace>GAZ</oboInOwl:hasOBONamespace>
        <oboInOwl:id>GAZ:00266166</oboInOwl:id>
        <rdfs:label>Reserva Biologica Manchon Guamuchal</rdfs:label>
    </owl:NamedIndividual>
    


    <!-- http://purl.obolibrary.org/obo/GAZ_00266168 -->

    <owl:NamedIndividual rdf:about="http://purl.obolibrary.org/obo/GAZ_00266168">
        <obo:RO_0001025 rdf:resource="http://purl.obolibrary.org/obo/GAZ_00068274"/>
        <obo:IAO_0000115>A protected area.</obo:IAO_0000115>
        <oboInOwl:hasOBONamespace>GAZ</oboInOwl:hasOBONamespace>
        <oboInOwl:id>GAZ:00266168</oboInOwl:id>
        <rdfs:label>Reserva Biologica Volcan Cerro Gordo</rdfs:label>
    </owl:NamedIndividual>
    


    <!-- http://purl.obolibrary.org/obo/GAZ_00266170 -->

    <owl:NamedIndividual rdf:about="http://purl.obolibrary.org/obo/GAZ_00266170">
        <obo:RO_0001025 rdf:resource="http://purl.obolibrary.org/obo/GAZ_00068272"/>
        <obo:IAO_0000115>A protected area.</obo:IAO_0000115>
        <oboInOwl:hasOBONamespace>GAZ</oboInOwl:hasOBONamespace>
        <oboInOwl:id>GAZ:00266170</oboInOwl:id>
        <rdfs:label>Biotopo Monterrico</rdfs:label>
    </owl:NamedIndividual>
    


    <!-- http://purl.obolibrary.org/obo/GAZ_00266171 -->

    <owl:NamedIndividual rdf:about="http://purl.obolibrary.org/obo/GAZ_00266171">
        <obo:RO_0001025 rdf:resource="http://purl.obolibrary.org/obo/GAZ_00068282"/>
        <obo:IAO_0000115>A protected area.</obo:IAO_0000115>
        <oboInOwl:hasOBONamespace>GAZ</oboInOwl:hasOBONamespace>
        <oboInOwl:id>GAZ:00266171</oboInOwl:id>
        <rdfs:label>Reserva Biologica Volcan Cruz Quemada</rdfs:label>
    </owl:NamedIndividual>
    


    <!-- http://purl.obolibrary.org/obo/GAZ_00266172 -->

    <owl:NamedIndividual rdf:about="http://purl.obolibrary.org/obo/GAZ_00266172">
        <obo:RO_0001025 rdf:resource="http://purl.obolibrary.org/obo/GAZ_00068284"/>
        <obo:IAO_0000115>A protected area.</obo:IAO_0000115>
        <oboInOwl:hasOBONamespace>GAZ</oboInOwl:hasOBONamespace>
        <oboInOwl:id>GAZ:00266172</oboInOwl:id>
        <rdfs:label>Reserva Biologica Volcan Cerro Redondo</rdfs:label>
    </owl:NamedIndividual>
    


    <!-- http://purl.obolibrary.org/obo/GAZ_00266173 -->

    <owl:NamedIndividual rdf:about="http://purl.obolibrary.org/obo/GAZ_00266173">
        <obo:RO_0001025 rdf:resource="http://purl.obolibrary.org/obo/GAZ_00000540"/>
        <obo:RO_0001025 rdf:resource="http://purl.obolibrary.org/obo/GAZ_00068275"/>
        <obo:IAO_0000115>A protected area.</obo:IAO_0000115>
        <oboInOwl:hasOBONamespace>GAZ</oboInOwl:hasOBONamespace>
        <oboInOwl:id>GAZ:00266173</oboInOwl:id>
        <rdfs:label>Reserva Biologica Volcan Jumaytepeque</rdfs:label>
    </owl:NamedIndividual>
    


    <!-- http://purl.obolibrary.org/obo/GAZ_00266174 -->

    <owl:NamedIndividual rdf:about="http://purl.obolibrary.org/obo/GAZ_00266174">
        <obo:RO_0001025 rdf:resource="http://purl.obolibrary.org/obo/GAZ_00068274"/>
        <obo:IAO_0000115>A protected area. Established 1955.</obo:IAO_0000115>
        <oboInOwl:hasOBONamespace>GAZ</oboInOwl:hasOBONamespace>
        <oboInOwl:id>GAZ:00266174</oboInOwl:id>
        <rdfs:label>Parque Nacional Laguna de El Pino</rdfs:label>
    </owl:NamedIndividual>
    


    <!-- http://purl.obolibrary.org/obo/GAZ_00266175 -->

    <owl:NamedIndividual rdf:about="http://purl.obolibrary.org/obo/GAZ_00266175">
        <obo:RO_0001025 rdf:resource="http://purl.obolibrary.org/obo/GAZ_00000549"/>
        <obo:IAO_0000115>A protected area.</obo:IAO_0000115>
        <oboInOwl:hasOBONamespace>GAZ</oboInOwl:hasOBONamespace>
        <oboInOwl:id>GAZ:00266175</oboInOwl:id>
        <rdfs:label>Parque Nacional Riscos de Momostenango</rdfs:label>
    </owl:NamedIndividual>
    


    <!-- http://purl.obolibrary.org/obo/GAZ_00266176 -->

    <owl:NamedIndividual rdf:about="http://purl.obolibrary.org/obo/GAZ_00266176">
        <obo:RO_0001025 rdf:resource="http://purl.obolibrary.org/obo/GAZ_00000549"/>
        <obo:IAO_0000115>A protected area.</obo:IAO_0000115>
        <oboInOwl:hasOBONamespace>GAZ</oboInOwl:hasOBONamespace>
        <oboInOwl:id>GAZ:00266176</oboInOwl:id>
        <rdfs:label>Reserva Biologica del Volcan Cuxliquel</rdfs:label>
    </owl:NamedIndividual>
    


    <!-- http://purl.obolibrary.org/obo/GAZ_00266177 -->

    <owl:NamedIndividual rdf:about="http://purl.obolibrary.org/obo/GAZ_00266177">
        <obo:RO_0001025 rdf:resource="http://purl.obolibrary.org/obo/GAZ_00266043"/>
        <obo:IAO_0000115>An island.</obo:IAO_0000115>
        <oboInOwl:hasOBONamespace>GAZ</oboInOwl:hasOBONamespace>
        <oboInOwl:id>GAZ:00266177</oboInOwl:id>
        <rdfs:label>Cayo Julio</rdfs:label>
    </owl:NamedIndividual>
    


    <!-- http://purl.obolibrary.org/obo/GAZ_00266178 -->

    <owl:NamedIndividual rdf:about="http://purl.obolibrary.org/obo/GAZ_00266178">
        <obo:RO_0001025 rdf:resource="http://purl.obolibrary.org/obo/GAZ_00266043"/>
        <obo:IAO_0000115>An island.</obo:IAO_0000115>
        <oboInOwl:hasOBONamespace>GAZ</oboInOwl:hasOBONamespace>
        <oboInOwl:id>GAZ:00266178</oboInOwl:id>
        <rdfs:label>Cayo Grande</rdfs:label>
    </owl:NamedIndividual>
    


    <!-- http://purl.obolibrary.org/obo/GAZ_00266179 -->

    <owl:NamedIndividual rdf:about="http://purl.obolibrary.org/obo/GAZ_00266179">
        <obo:RO_0001025 rdf:resource="http://purl.obolibrary.org/obo/GAZ_00266043"/>
        <obo:IAO_0000115>An island.</obo:IAO_0000115>
        <oboInOwl:hasOBONamespace>GAZ</oboInOwl:hasOBONamespace>
        <oboInOwl:id>GAZ:00266179</oboInOwl:id>
        <rdfs:label>Cayo Palomo</rdfs:label>
    </owl:NamedIndividual>
    


    <!-- http://purl.obolibrary.org/obo/GAZ_00266180 -->

    <owl:NamedIndividual rdf:about="http://purl.obolibrary.org/obo/GAZ_00266180">
        <obo:RO_0001025 rdf:resource="http://purl.obolibrary.org/obo/GAZ_00266043"/>
        <obo:IAO_0000115>An island.</obo:IAO_0000115>
        <oboInOwl:hasOBONamespace>GAZ</oboInOwl:hasOBONamespace>
        <oboInOwl:id>GAZ:00266180</oboInOwl:id>
        <rdfs:label>Cuatro Cayos</rdfs:label>
    </owl:NamedIndividual>
    


    <!-- http://purl.obolibrary.org/obo/GAZ_00266181 -->

    <owl:NamedIndividual rdf:about="http://purl.obolibrary.org/obo/GAZ_00266181">
        <obo:RO_0001025 rdf:resource="http://purl.obolibrary.org/obo/GAZ_00000477"/>
        <obo:IAO_0000115>A protected area. Located along the Pacific coast of Escuintla in Guatemala.</obo:IAO_0000115>
        <oboInOwl:hasOBONamespace>GAZ</oboInOwl:hasOBONamespace>
        <oboInOwl:id>GAZ:00266181</oboInOwl:id>
        <rdfs:label>Parque Nacional Sipacate-Naranjo</rdfs:label>
    </owl:NamedIndividual>
    


    <!-- http://purl.obolibrary.org/obo/GAZ_00266182 -->

    <owl:NamedIndividual rdf:about="http://purl.obolibrary.org/obo/GAZ_00266182">
        <obo:RO_0001025 rdf:resource="http://purl.obolibrary.org/obo/GAZ_00068105"/>
        <obo:IAO_0000115>A crater lake in the municipality of San Vicente Pacaya, Escuintla, Guatemala. It is located approximately 6 km south of Lake Amatitlan and 3 km north of the currently active vent of the Pacaya volcano.</obo:IAO_0000115>
        <oboInOwl:hasOBONamespace>GAZ</oboInOwl:hasOBONamespace>
        <oboInOwl:id>GAZ:00266182</oboInOwl:id>
        <rdfs:label>Laguna de Calderas</rdfs:label>
    </owl:NamedIndividual>
    


    <!-- http://purl.obolibrary.org/obo/GAZ_00266185 -->

    <owl:NamedIndividual rdf:about="http://purl.obolibrary.org/obo/GAZ_00266185">
        <obo:RO_0001025 rdf:resource="http://purl.obolibrary.org/obo/GAZ_00068115"/>
        <obo:IAO_0000115>A reinforced concrete gravity dam and power plant spanning the Las Vacas River near the village of San Antonio Las Flores. Constructed 1998-2002.</obo:IAO_0000115>
        <oboInOwl:hasOBONamespace>GAZ</oboInOwl:hasOBONamespace>
        <oboInOwl:id>GAZ:00266185</oboInOwl:id>
        <rdfs:label>Planta Hidroelectrica Rio Las Vacas</rdfs:label>
    </owl:NamedIndividual>
    


    <!-- http://purl.obolibrary.org/obo/GAZ_00266186 -->

    <owl:NamedIndividual rdf:about="http://purl.obolibrary.org/obo/GAZ_00266186">
        <obo:RO_0001025 rdf:resource="http://purl.obolibrary.org/obo/GAZ_00068172"/>
        <obo:IAO_0000115>A cave. An archeological site.</obo:IAO_0000115>
        <oboInOwl:hasOBONamespace>GAZ</oboInOwl:hasOBONamespace>
        <oboInOwl:id>GAZ:00266186</oboInOwl:id>
        <rdfs:label>Naj Tunich Cave</rdfs:label>
    </owl:NamedIndividual>
    


    <!-- http://purl.obolibrary.org/obo/GAZ_00266187 -->

    <owl:NamedIndividual rdf:about="http://purl.obolibrary.org/obo/GAZ_00266187">
        <obo:RO_0001025 rdf:resource="http://purl.obolibrary.org/obo/GAZ_00000495"/>
        <obo:IAO_0000115>A protected area. Established 1972.</obo:IAO_0000115>
        <oboInOwl:hasOBONamespace>GAZ</oboInOwl:hasOBONamespace>
        <oboInOwl:id>GAZ:00266187</oboInOwl:id>
        <rdfs:label>Parque Nacional Cuevas del Silvino</rdfs:label>
    </owl:NamedIndividual>
    


    <!-- http://purl.obolibrary.org/obo/GAZ_00266188 -->

    <owl:NamedIndividual rdf:about="http://purl.obolibrary.org/obo/GAZ_00266188">
        <obo:RO_0001025 rdf:resource="http://purl.obolibrary.org/obo/GAZ_00266187"/>
        <obo:IAO_0000115>Karst caves.</obo:IAO_0000115>
        <oboInOwl:hasOBONamespace>GAZ</oboInOwl:hasOBONamespace>
        <oboInOwl:id>GAZ:00266188</oboInOwl:id>
        <rdfs:label>Cuevas del Silvino</rdfs:label>
    </owl:NamedIndividual>
    


    <!-- http://purl.obolibrary.org/obo/GAZ_00266190 -->

    <owl:NamedIndividual rdf:about="http://purl.obolibrary.org/obo/GAZ_00266190">
        <obo:RO_0001025 rdf:resource="http://purl.obolibrary.org/obo/GAZ_00068182"/>
        <obo:IAO_0000115>A natural cave in the municipality of Flores in Guatemala.</obo:IAO_0000115>
        <oboInOwl:hasOBONamespace>GAZ</oboInOwl:hasOBONamespace>
        <oboInOwl:id>GAZ:00266190</oboInOwl:id>
        <rdfs:label>Actun Can</rdfs:label>
    </owl:NamedIndividual>
    


    <!-- http://purl.obolibrary.org/obo/GAZ_00266191 -->

    <owl:NamedIndividual rdf:about="http://purl.obolibrary.org/obo/GAZ_00266191">
        <obo:RO_0001025 rdf:resource="http://purl.obolibrary.org/obo/GAZ_00068182"/>
        <obo:IAO_0000115>A cave.</obo:IAO_0000115>
        <oboInOwl:hasOBONamespace>GAZ</oboInOwl:hasOBONamespace>
        <oboInOwl:id>GAZ:00266191</oboInOwl:id>
        <rdfs:label>Jobitzinaj Cave</rdfs:label>
    </owl:NamedIndividual>
    


    <!-- http://purl.obolibrary.org/obo/GAZ_00266192 -->

    <owl:NamedIndividual rdf:about="http://purl.obolibrary.org/obo/GAZ_00266192">
        <obo:RO_0001025 rdf:resource="http://purl.obolibrary.org/obo/GAZ_00000508"/>
        <obo:IAO_0000115>A cave.</obo:IAO_0000115>
        <oboInOwl:hasOBONamespace>GAZ</oboInOwl:hasOBONamespace>
        <oboInOwl:id>GAZ:00266192</oboInOwl:id>
        <rdfs:label>Grutas de Uaxactun</rdfs:label>
    </owl:NamedIndividual>
    


    <!-- http://purl.obolibrary.org/obo/GAZ_00266193 -->

    <owl:NamedIndividual rdf:about="http://purl.obolibrary.org/obo/GAZ_00266193">
        <obo:RO_0001025 rdf:resource="http://purl.obolibrary.org/obo/GAZ_00000508"/>
        <obo:IAO_0000115>A cave.</obo:IAO_0000115>
        <oboInOwl:hasOBONamespace>GAZ</oboInOwl:hasOBONamespace>
        <oboInOwl:id>GAZ:00266193</oboInOwl:id>
        <rdfs:label>Ixobel Cave</rdfs:label>
    </owl:NamedIndividual>
    


    <!-- http://purl.obolibrary.org/obo/GAZ_00266194 -->

    <owl:NamedIndividual rdf:about="http://purl.obolibrary.org/obo/GAZ_00266194">
        <obo:RO_0001025 rdf:resource="http://purl.obolibrary.org/obo/GAZ_00068088"/>
        <obo:IAO_0000115>A cave.</obo:IAO_0000115>
        <oboInOwl:hasOBONamespace>GAZ</oboInOwl:hasOBONamespace>
        <oboInOwl:id>GAZ:00266194</oboInOwl:id>
        <rdfs:label>Las Minas Cave</rdfs:label>
    </owl:NamedIndividual>
    


    <!-- http://purl.obolibrary.org/obo/GAZ_00266195 -->

    <owl:NamedIndividual rdf:about="http://purl.obolibrary.org/obo/GAZ_00266195">
        <obo:RO_0001025 rdf:resource="http://purl.obolibrary.org/obo/GAZ_00068059"/>
        <obo:IAO_0000115>A cave.</obo:IAO_0000115>
        <oboInOwl:hasOBONamespace>GAZ</oboInOwl:hasOBONamespace>
        <oboInOwl:id>GAZ:00266195</oboInOwl:id>
        <rdfs:label>K&apos;an Ba Cave</rdfs:label>
    </owl:NamedIndividual>
    


    <!-- http://purl.obolibrary.org/obo/GAZ_00266196 -->

    <owl:NamedIndividual rdf:about="http://purl.obolibrary.org/obo/GAZ_00266196">
        <obo:RO_0001025 rdf:resource="http://purl.obolibrary.org/obo/GAZ_00067906"/>
        <obo:IAO_0000115>A cave.</obo:IAO_0000115>
        <oboInOwl:hasOBONamespace>GAZ</oboInOwl:hasOBONamespace>
        <oboInOwl:id>GAZ:00266196</oboInOwl:id>
        <rdfs:label>B&apos;onb&apos;il Pek Cave</rdfs:label>
    </owl:NamedIndividual>
    


    <!-- http://purl.obolibrary.org/obo/GAZ_00266197 -->

    <owl:NamedIndividual rdf:about="http://purl.obolibrary.org/obo/GAZ_00266197">
        <obo:RO_0001025 rdf:resource="http://purl.obolibrary.org/obo/GAZ_00000434"/>
        <obo:IAO_0000115>A cave.</obo:IAO_0000115>
        <oboInOwl:hasOBONamespace>GAZ</oboInOwl:hasOBONamespace>
        <oboInOwl:id>GAZ:00266197</oboInOwl:id>
        <rdfs:label>Chicoy Cave</rdfs:label>
    </owl:NamedIndividual>
    


    <!-- http://purl.obolibrary.org/obo/GAZ_00266198 -->

    <owl:NamedIndividual rdf:about="http://purl.obolibrary.org/obo/GAZ_00266198">
        <obo:RO_0001025 rdf:resource="http://purl.obolibrary.org/obo/GAZ_00000494"/>
        <obo:IAO_0000115>A small mountain range northeast of the Sierra de las Minas, near Puerto Barrios.</obo:IAO_0000115>
        <oboInOwl:hasOBONamespace>GAZ</oboInOwl:hasOBONamespace>
        <oboInOwl:id>GAZ:00266198</oboInOwl:id>
        <rdfs:label>Sierra del Mico</rdfs:label>
    </owl:NamedIndividual>
    


    <!-- http://purl.obolibrary.org/obo/GAZ_00266199 -->

    <owl:NamedIndividual rdf:about="http://purl.obolibrary.org/obo/GAZ_00266199">
        <obo:RO_0001025 rdf:resource="http://purl.obolibrary.org/obo/GAZ_00000508"/>
        <obo:RO_0001025 rdf:resource="http://purl.obolibrary.org/obo/GAZ_00266102"/>
        <obo:IAO_0000115>A protected area. Located in the tropical rain forest in the north west of Guatemala.</obo:IAO_0000115>
        <oboInOwl:hasOBONamespace>GAZ</oboInOwl:hasOBONamespace>
        <oboInOwl:id>GAZ:00266199</oboInOwl:id>
        <rdfs:label>Parque Nacional Sierra del Lacandon</rdfs:label>
    </owl:NamedIndividual>
    


    <!-- http://purl.obolibrary.org/obo/GAZ_00266201 -->

    <owl:NamedIndividual rdf:about="http://purl.obolibrary.org/obo/GAZ_00266201">
        <obo:RO_0001025 rdf:resource="http://purl.obolibrary.org/obo/GAZ_00000508"/>
        <obo:IAO_0000115>An archaeological site of the Maya civilization located along an escarpment in the Peten department of Guatemala.</obo:IAO_0000115>
        <oboInOwl:hasOBONamespace>GAZ</oboInOwl:hasOBONamespace>
        <oboInOwl:id>GAZ:00266201</oboInOwl:id>
        <rdfs:label>Tamarindito</rdfs:label>
    </owl:NamedIndividual>
    


    <!-- http://purl.obolibrary.org/obo/GAZ_00266202 -->

    <owl:NamedIndividual rdf:about="http://purl.obolibrary.org/obo/GAZ_00266202">
        <obo:RO_0001025 rdf:resource="http://purl.obolibrary.org/obo/GAZ_00068316"/>
        <obo:IAO_0000115>An archeological site. A Preclassic Southern Maya site whose developmental emphasis was from ca. 1000 BC to AD 200.</obo:IAO_0000115>
        <oboInOwl:hasOBONamespace>GAZ</oboInOwl:hasOBONamespace>
        <oboInOwl:id>GAZ:00266202</oboInOwl:id>
        <rdfs:label>Chocola</rdfs:label>
    </owl:NamedIndividual>
    


    <!-- http://purl.obolibrary.org/obo/GAZ_00266203 -->

    <owl:NamedIndividual rdf:about="http://purl.obolibrary.org/obo/GAZ_00266203">
        <obo:RO_0001025 rdf:resource="http://purl.obolibrary.org/obo/GAZ_00266062"/>
        <obo:IAO_0000115>A pre-Columbian Maya civilization archaeological site, situated in the Peten Basin region of the southern Maya lowlands.</obo:IAO_0000115>
        <oboInOwl:hasOBONamespace>GAZ</oboInOwl:hasOBONamespace>
        <oboInOwl:id>GAZ:00266203</oboInOwl:id>
        <rdfs:label>Ixkun</rdfs:label>
    </owl:NamedIndividual>
    


    <!-- http://purl.obolibrary.org/obo/GAZ_00266204 -->

    <owl:NamedIndividual rdf:about="http://purl.obolibrary.org/obo/GAZ_00266204">
        <obo:RO_0001025 rdf:resource="http://purl.obolibrary.org/obo/GAZ_00005154"/>
        <obo:IAO_0000115>A Pre-Columbian site of the Maya civilization that was primarily occupied from 1500BC to 1200AD.</obo:IAO_0000115>
        <oboInOwl:hasOBONamespace>GAZ</oboInOwl:hasOBONamespace>
        <oboInOwl:id>GAZ:00266204</oboInOwl:id>
        <rdfs:label>Kaminaljuyu</rdfs:label>
    </owl:NamedIndividual>
    


    <!-- http://purl.obolibrary.org/obo/GAZ_00266205 -->

    <owl:NamedIndividual rdf:about="http://purl.obolibrary.org/obo/GAZ_00266205">
        <obo:RO_0001025 rdf:resource="http://purl.obolibrary.org/obo/GAZ_00000439"/>
        <obo:IAO_0000115>An archaeological site in the north east of the Chimaltenango department of Guatemala, some 50 km to the north of Guatemala City and 4km from the junction of the rivers Pixcaya and Montagua.</obo:IAO_0000115>
        <oboInOwl:hasOBONamespace>GAZ</oboInOwl:hasOBONamespace>
        <oboInOwl:id>GAZ:00266205</oboInOwl:id>
        <rdfs:label>Mixco Viejo</rdfs:label>
    </owl:NamedIndividual>
    


    <!-- http://purl.obolibrary.org/obo/GAZ_00266206 -->

    <owl:NamedIndividual rdf:about="http://purl.obolibrary.org/obo/GAZ_00266206">
        <obo:RO_0001025 rdf:resource="http://purl.obolibrary.org/obo/GAZ_00266060"/>
        <obo:IAO_0000115>An archaeological site of the pre-Columbian Maya civilization, situated at the northeastern perimeter of the Mirador Basin region in the southern Maya lowlands, now in the modern-day Department of El Peten.</obo:IAO_0000115>
        <oboInOwl:hasOBONamespace>GAZ</oboInOwl:hasOBONamespace>
        <oboInOwl:id>GAZ:00266206</oboInOwl:id>
        <rdfs:label>Naachtun</rdfs:label>
    </owl:NamedIndividual>
    


    <!-- http://purl.obolibrary.org/obo/GAZ_00266207 -->

    <owl:NamedIndividual rdf:about="http://purl.obolibrary.org/obo/GAZ_00266207">
        <obo:RO_0001025 rdf:resource="http://purl.obolibrary.org/obo/GAZ_00266086"/>
        <obo:IAO_0000115>A pre-Columbian archeological site.</obo:IAO_0000115>
        <oboInOwl:hasOBONamespace>GAZ</oboInOwl:hasOBONamespace>
        <oboInOwl:id>GAZ:00266207</oboInOwl:id>
        <rdfs:label>Sak Ha Witznal</rdfs:label>
    </owl:NamedIndividual>
    


    <!-- http://purl.obolibrary.org/obo/GAZ_00266208 -->

    <owl:NamedIndividual rdf:about="http://purl.obolibrary.org/obo/GAZ_00266208">
        <obo:RO_0001025 rdf:resource="http://purl.obolibrary.org/obo/GAZ_00000508"/>
        <obo:IAO_0000115>A small pre-Columbian Maya archaeological site located in the Department of Peten in northern Guatemala, northeast of Tikal and roughly fifty miles from the nearest settlement.</obo:IAO_0000115>
        <oboInOwl:hasOBONamespace>GAZ</oboInOwl:hasOBONamespace>
        <oboInOwl:id>GAZ:00266208</oboInOwl:id>
        <rdfs:label>San Bartolo</rdfs:label>
    </owl:NamedIndividual>
    


    <!-- http://purl.obolibrary.org/obo/GAZ_00266209 -->

    <owl:NamedIndividual rdf:about="http://purl.obolibrary.org/obo/GAZ_00266209">
        <obo:RO_0001025 rdf:resource="http://purl.obolibrary.org/obo/GAZ_00000508"/>
        <obo:IAO_0000115>A pre-Columbian Maya archaeological site in northern Guatemala. The site of Zacpeten occupies a peninsula on Lake Salpeten.</obo:IAO_0000115>
        <oboInOwl:hasOBONamespace>GAZ</oboInOwl:hasOBONamespace>
        <oboInOwl:id>GAZ:00266209</oboInOwl:id>
        <rdfs:label>Zacpeten</rdfs:label>
    </owl:NamedIndividual>
    


    <!-- http://purl.obolibrary.org/obo/GAZ_00266210 -->

    <owl:NamedIndividual rdf:about="http://purl.obolibrary.org/obo/GAZ_00266210">
        <obo:RO_0001025 rdf:resource="http://purl.obolibrary.org/obo/GAZ_00000508"/>
        <obo:IAO_0000115>A pre-Columbian Maya archaeological site located south of the San Pedro Martir river in the Peten department of Guatemala.</obo:IAO_0000115>
        <oboInOwl:hasOBONamespace>GAZ</oboInOwl:hasOBONamespace>
        <oboInOwl:id>GAZ:00266210</oboInOwl:id>
        <rdfs:label>Zapote Bobal</rdfs:label>
    </owl:NamedIndividual>
    


    <!-- http://purl.obolibrary.org/obo/GAZ_00266211 -->

    <owl:NamedIndividual rdf:about="http://purl.obolibrary.org/obo/GAZ_00266211">
        <obo:RO_0001025 rdf:resource="http://purl.obolibrary.org/obo/GAZ_00068059"/>
        <obo:IAO_0000115>A protected area.</obo:IAO_0000115>
        <oboInOwl:hasOBONamespace>GAZ</oboInOwl:hasOBONamespace>
        <oboInOwl:id>GAZ:00266211</oboInOwl:id>
        <rdfs:label>Semuc Champey</rdfs:label>
    </owl:NamedIndividual>
    


    <!-- http://purl.obolibrary.org/obo/GAZ_00266212 -->

    <owl:NamedIndividual rdf:about="http://purl.obolibrary.org/obo/GAZ_00266212">
        <rdf:type rdf:resource="http://purl.obolibrary.org/obo/ENVO_00000305"/>
        <obo:RO_0001025 rdf:resource="http://purl.obolibrary.org/obo/GAZ_00000494"/>
        <obo:IAO_0000115>A cape. The E limit of the Bahia de Amatique.</obo:IAO_0000115>
        <oboInOwl:hasOBONamespace>GAZ</oboInOwl:hasOBONamespace>
        <oboInOwl:id>GAZ:00266212</oboInOwl:id>
        <rdfs:label>Cabo de Tres Puntas</rdfs:label>
    </owl:NamedIndividual>
    


    <!-- http://purl.obolibrary.org/obo/GAZ_00266214 -->

    <owl:NamedIndividual rdf:about="http://purl.obolibrary.org/obo/GAZ_00266214">
        <obo:RO_0001025 rdf:resource="http://purl.obolibrary.org/obo/GAZ_00000529"/>
        <obo:IAO_0000115>A river.</obo:IAO_0000115>
        <oboInOwl:hasOBONamespace>GAZ</oboInOwl:hasOBONamespace>
        <oboInOwl:id>GAZ:00266214</oboInOwl:id>
        <rdfs:label>Rio Cabuz</rdfs:label>
    </owl:NamedIndividual>
    


    <!-- http://purl.obolibrary.org/obo/GAZ_00266215 -->

    <owl:NamedIndividual rdf:about="http://purl.obolibrary.org/obo/GAZ_00266215">
        <obo:RO_0001025 rdf:resource="http://purl.obolibrary.org/obo/GAZ_00000529"/>
        <obo:IAO_0000115>A river. Discharges to the Pacific Ocean.</obo:IAO_0000115>
        <oboInOwl:hasOBONamespace>GAZ</oboInOwl:hasOBONamespace>
        <oboInOwl:id>GAZ:00266215</oboInOwl:id>
        <rdfs:label>Rio Nuhuatan</rdfs:label>
    </owl:NamedIndividual>
    


    <!-- http://purl.obolibrary.org/obo/GAZ_00266225 -->

    <owl:NamedIndividual rdf:about="http://purl.obolibrary.org/obo/GAZ_00266225">
        <obo:RO_0001025 rdf:resource="http://purl.obolibrary.org/obo/GAZ_00000545"/>
        <obo:IAO_0000115>A river in Southwest Guatemala. Its sources are located in the Sierra Madre range, on the slopes of the Santo Tomas volcano in the department of Suchitepequez. It flows southwards through the coastal lowlands of Suchitepequez to the Pacific Ocean.</obo:IAO_0000115>
        <oboInOwl:hasOBONamespace>GAZ</oboInOwl:hasOBONamespace>
        <oboInOwl:id>GAZ:00266225</oboInOwl:id>
        <rdfs:label>Rio Ican</rdfs:label>
    </owl:NamedIndividual>
    


    <!-- http://purl.obolibrary.org/obo/GAZ_00266230 -->

    <owl:NamedIndividual rdf:about="http://purl.obolibrary.org/obo/GAZ_00266230">
        <obo:RO_0001025 rdf:resource="http://purl.obolibrary.org/obo/GAZ_00000545"/>
        <obo:IAO_0000115>A river.</obo:IAO_0000115>
        <oboInOwl:hasOBONamespace>GAZ</oboInOwl:hasOBONamespace>
        <oboInOwl:id>GAZ:00266230</oboInOwl:id>
        <rdfs:label>Rio Cutzan</rdfs:label>
    </owl:NamedIndividual>
    


    <!-- http://purl.obolibrary.org/obo/GAZ_00266232 -->

    <owl:NamedIndividual rdf:about="http://purl.obolibrary.org/obo/GAZ_00266232">
        <obo:IAO_0000115>A river.</obo:IAO_0000115>
        <oboInOwl:hasOBONamespace>GAZ</oboInOwl:hasOBONamespace>
        <oboInOwl:id>GAZ:00266232</oboInOwl:id>
        <rdfs:label>Rio Quixaya</rdfs:label>
    </owl:NamedIndividual>
    


    <!-- http://purl.obolibrary.org/obo/GAZ_00266237 -->

    <owl:NamedIndividual rdf:about="http://purl.obolibrary.org/obo/GAZ_00266237">
        <obo:RO_0001025 rdf:resource="http://purl.obolibrary.org/obo/GAZ_00000477"/>
        <obo:IAO_0000115>A river in the south of Guatemala. Its sources are located in the Sierra Madre range, on the southern slopes of the Volcan de Fuego in the departments of Sacatepequez and Escuintla. The river flows southwards through the coastal lowlands of Escuintla to the Pacific Ocean.</obo:IAO_0000115>
        <oboInOwl:hasOBONamespace>GAZ</oboInOwl:hasOBONamespace>
        <oboInOwl:id>GAZ:00266237</oboInOwl:id>
        <rdfs:label>Rio Achiguate</rdfs:label>
    </owl:NamedIndividual>
    


    <!-- http://purl.obolibrary.org/obo/GAZ_00266239 -->

    <owl:NamedIndividual rdf:about="http://purl.obolibrary.org/obo/GAZ_00266239">
        <obo:RO_0001025 rdf:resource="http://purl.obolibrary.org/obo/GAZ_00000477"/>
        <obo:IAO_0000115>A river in southwest Guatemala. Its sources are located south of Lake Amatitlan in the department of Guatemala. It flows southwards through the coastal lowlands of Escuintla and Santa Rosa to the Pacific Ocean.</obo:IAO_0000115>
        <oboInOwl:hasOBONamespace>GAZ</oboInOwl:hasOBONamespace>
        <oboInOwl:id>GAZ:00266239</oboInOwl:id>
        <rdfs:label>Rio Maria Linda</rdfs:label>
    </owl:NamedIndividual>
    


    <!-- http://purl.obolibrary.org/obo/GAZ_00266242 -->

    <owl:NamedIndividual rdf:about="http://purl.obolibrary.org/obo/GAZ_00266242">
        <obo:RO_0001025 rdf:resource="http://purl.obolibrary.org/obo/GAZ_00000477"/>
        <obo:IAO_0000115>A river.</obo:IAO_0000115>
        <oboInOwl:hasOBONamespace>GAZ</oboInOwl:hasOBONamespace>
        <oboInOwl:id>GAZ:00266242</oboInOwl:id>
        <rdfs:label>Rio Naranjo</rdfs:label>
    </owl:NamedIndividual>
    


    <!-- http://purl.obolibrary.org/obo/GAZ_00266243 -->

    <owl:NamedIndividual rdf:about="http://purl.obolibrary.org/obo/GAZ_00266243">
        <obo:RO_0001025 rdf:resource="http://purl.obolibrary.org/obo/GAZ_00000540"/>
        <obo:IAO_0000115>A river in Southern Guatemala. Its sources are located in the mountains in the southeast of the department of Santa Rosa. From there it flows past the town Cuilapa through the coastal plains of Santa Rosa into the Laguna de Sipacate and then into the Pacific Ocean.</obo:IAO_0000115>
        <oboInOwl:hasOBONamespace>GAZ</oboInOwl:hasOBONamespace>
        <oboInOwl:id>GAZ:00266243</oboInOwl:id>
        <rdfs:label>Rio Los Esclavos</rdfs:label>
    </owl:NamedIndividual>
    


    <!-- http://purl.obolibrary.org/obo/GAZ_00266244 -->

    <owl:NamedIndividual rdf:about="http://purl.obolibrary.org/obo/GAZ_00266244">
        <obo:RO_0001025 rdf:resource="http://purl.obolibrary.org/obo/GAZ_00266243"/>
        <oboInOwl:hasOBONamespace>GAZ</oboInOwl:hasOBONamespace>
        <oboInOwl:id>GAZ:00266244</oboInOwl:id>
        <rdfs:label>Laguna de Sipacate</rdfs:label>
    </owl:NamedIndividual>
    


    <!-- http://purl.obolibrary.org/obo/GAZ_00266245 -->

    <owl:NamedIndividual rdf:about="http://purl.obolibrary.org/obo/GAZ_00266245">
        <obo:RO_0001025 rdf:resource="http://purl.obolibrary.org/obo/GAZ_00000499"/>
        <obo:IAO_0000115>A river.</obo:IAO_0000115>
        <oboInOwl:hasOBONamespace>GAZ</oboInOwl:hasOBONamespace>
        <oboInOwl:id>GAZ:00266245</oboInOwl:id>
        <rdfs:label>Rio Pulula</rdfs:label>
    </owl:NamedIndividual>
    


    <!-- http://purl.obolibrary.org/obo/GAZ_00266246 -->

    <owl:NamedIndividual rdf:about="http://purl.obolibrary.org/obo/GAZ_00266246">
        <obo:RO_0001025 rdf:resource="http://purl.obolibrary.org/obo/GAZ_00000499"/>
        <obo:IAO_0000115>A river.</obo:IAO_0000115>
        <oboInOwl:hasOBONamespace>GAZ</oboInOwl:hasOBONamespace>
        <oboInOwl:id>GAZ:00266246</oboInOwl:id>
        <rdfs:label>Rio Grande de Mita</rdfs:label>
    </owl:NamedIndividual>
    


    <!-- http://purl.obolibrary.org/obo/GAZ_00266247 -->

    <owl:NamedIndividual rdf:about="http://purl.obolibrary.org/obo/GAZ_00266247">
        <obo:RO_0001025 rdf:resource="http://purl.obolibrary.org/obo/GAZ_00000499"/>
        <obo:IAO_0000115>A river.</obo:IAO_0000115>
        <oboInOwl:hasOBONamespace>GAZ</oboInOwl:hasOBONamespace>
        <oboInOwl:id>GAZ:00266247</oboInOwl:id>
        <rdfs:label>Rio Mongoy</rdfs:label>
    </owl:NamedIndividual>
    


    <!-- http://purl.obolibrary.org/obo/GAZ_00266248 -->

    <owl:NamedIndividual rdf:about="http://purl.obolibrary.org/obo/GAZ_00266248">
        <obo:RO_0001025 rdf:resource="http://purl.obolibrary.org/obo/GAZ_00000499"/>
        <obo:IAO_0000115>A river.</obo:IAO_0000115>
        <oboInOwl:hasOBONamespace>GAZ</oboInOwl:hasOBONamespace>
        <oboInOwl:id>GAZ:00266248</oboInOwl:id>
        <rdfs:label>Rio Salada</rdfs:label>
    </owl:NamedIndividual>
    


    <!-- http://purl.obolibrary.org/obo/GAZ_00266249 -->

    <owl:NamedIndividual rdf:about="http://purl.obolibrary.org/obo/GAZ_00266249">
        <obo:RO_0001025 rdf:resource="http://purl.obolibrary.org/obo/GAZ_00000494"/>
        <obo:IAO_0000115>A river. Discharges to the Gulf of Honduras.</obo:IAO_0000115>
        <oboInOwl:hasOBONamespace>GAZ</oboInOwl:hasOBONamespace>
        <oboInOwl:id>GAZ:00266249</oboInOwl:id>
        <rdfs:label>Rio San Francisco</rdfs:label>
    </owl:NamedIndividual>
    


    <!-- http://purl.obolibrary.org/obo/GAZ_00266254 -->

    <owl:NamedIndividual rdf:about="http://purl.obolibrary.org/obo/GAZ_00266254">
        <obo:IAO_0000115>A river.</obo:IAO_0000115>
        <oboInOwl:hasOBONamespace>GAZ</oboInOwl:hasOBONamespace>
        <oboInOwl:id>GAZ:00266254</oboInOwl:id>
        <rdfs:label>Rio Los Platanos</rdfs:label>
    </owl:NamedIndividual>
    


    <!-- http://purl.obolibrary.org/obo/GAZ_00266255 -->

    <owl:NamedIndividual rdf:about="http://purl.obolibrary.org/obo/GAZ_00266255">
        <obo:RO_0001025 rdf:resource="http://purl.obolibrary.org/obo/GAZ_00000439"/>
        <obo:IAO_0000115>A river.</obo:IAO_0000115>
        <oboInOwl:hasOBONamespace>GAZ</oboInOwl:hasOBONamespace>
        <oboInOwl:id>GAZ:00266255</oboInOwl:id>
        <rdfs:label>Rio Pixcaya</rdfs:label>
    </owl:NamedIndividual>
    


    <!-- http://purl.obolibrary.org/obo/GAZ_00266256 -->

    <owl:NamedIndividual rdf:about="http://purl.obolibrary.org/obo/GAZ_00266256">
        <obo:RO_0001025 rdf:resource="http://purl.obolibrary.org/obo/GAZ_00000517"/>
        <obo:IAO_0000115>A river.</obo:IAO_0000115>
        <oboInOwl:hasOBONamespace>GAZ</oboInOwl:hasOBONamespace>
        <oboInOwl:id>GAZ:00266256</oboInOwl:id>
        <rdfs:label>Rio Tzepela</rdfs:label>
    </owl:NamedIndividual>
    


    <!-- http://purl.obolibrary.org/obo/GAZ_00266258 -->

    <owl:NamedIndividual rdf:about="http://purl.obolibrary.org/obo/GAZ_00266258">
        <obo:RO_0001025 rdf:resource="http://purl.obolibrary.org/obo/GAZ_00000494"/>
        <obo:IAO_0000115>A river.</obo:IAO_0000115>
        <oboInOwl:hasOBONamespace>GAZ</oboInOwl:hasOBONamespace>
        <oboInOwl:id>GAZ:00266258</oboInOwl:id>
        <rdfs:label>Rio Tinagas</rdfs:label>
    </owl:NamedIndividual>
    


    <!-- http://purl.obolibrary.org/obo/GAZ_00266259 -->

    <owl:NamedIndividual rdf:about="http://purl.obolibrary.org/obo/GAZ_00266259">
        <obo:RO_0001025 rdf:resource="http://purl.obolibrary.org/obo/GAZ_00000494"/>
        <obo:IAO_0000115>A river.</obo:IAO_0000115>
        <oboInOwl:hasOBONamespace>GAZ</oboInOwl:hasOBONamespace>
        <oboInOwl:id>GAZ:00266259</oboInOwl:id>
        <rdfs:label>Rio Zarco</rdfs:label>
    </owl:NamedIndividual>
    


    <!-- http://purl.obolibrary.org/obo/GAZ_00266260 -->

    <owl:NamedIndividual rdf:about="http://purl.obolibrary.org/obo/GAZ_00266260">
        <obo:RO_0001025 rdf:resource="http://purl.obolibrary.org/obo/GAZ_00000430"/>
        <obo:IAO_0000115>A river.</obo:IAO_0000115>
        <oboInOwl:hasOBONamespace>GAZ</oboInOwl:hasOBONamespace>
        <oboInOwl:id>GAZ:00266260</oboInOwl:id>
        <rdfs:label>Rio Boca Nueva</rdfs:label>
    </owl:NamedIndividual>
    


    <!-- http://purl.obolibrary.org/obo/GAZ_00266261 -->

    <owl:NamedIndividual rdf:about="http://purl.obolibrary.org/obo/GAZ_00266261">
        <obo:RO_0001025 rdf:resource="http://purl.obolibrary.org/obo/GAZ_00000494"/>
        <obo:IAO_0000115>A river.</obo:IAO_0000115>
        <oboInOwl:hasOBONamespace>GAZ</oboInOwl:hasOBONamespace>
        <oboInOwl:id>GAZ:00266261</oboInOwl:id>
        <rdfs:label>Rio Oscuro</rdfs:label>
    </owl:NamedIndividual>
    


    <!-- http://purl.obolibrary.org/obo/GAZ_00266262 -->

    <owl:NamedIndividual rdf:about="http://purl.obolibrary.org/obo/GAZ_00266262">
        <obo:RO_0001025 rdf:resource="http://purl.obolibrary.org/obo/GAZ_00000494"/>
        <obo:IAO_0000115>A river.</obo:IAO_0000115>
        <oboInOwl:hasOBONamespace>GAZ</oboInOwl:hasOBONamespace>
        <oboInOwl:id>GAZ:00266262</oboInOwl:id>
        <rdfs:label>Rio Chinebal</rdfs:label>
    </owl:NamedIndividual>
    


    <!-- http://purl.obolibrary.org/obo/GAZ_00266263 -->

    <owl:NamedIndividual rdf:about="http://purl.obolibrary.org/obo/GAZ_00266263">
        <obo:RO_0001025 rdf:resource="http://purl.obolibrary.org/obo/GAZ_00000494"/>
        <obo:IAO_0000115>A river.</obo:IAO_0000115>
        <oboInOwl:hasOBONamespace>GAZ</oboInOwl:hasOBONamespace>
        <oboInOwl:id>GAZ:00266263</oboInOwl:id>
        <rdfs:label>Rio Tunico</rdfs:label>
    </owl:NamedIndividual>
    


    <!-- http://purl.obolibrary.org/obo/GAZ_00266264 -->

    <owl:NamedIndividual rdf:about="http://purl.obolibrary.org/obo/GAZ_00266264">
        <obo:RO_0001025 rdf:resource="http://purl.obolibrary.org/obo/GAZ_00000508"/>
        <obo:IAO_0000115>A river.</obo:IAO_0000115>
        <oboInOwl:hasOBONamespace>GAZ</oboInOwl:hasOBONamespace>
        <oboInOwl:id>GAZ:00266264</oboInOwl:id>
        <rdfs:label>Arrayo Sal Puedes</rdfs:label>
    </owl:NamedIndividual>
    


    <!-- http://purl.obolibrary.org/obo/GAZ_00266266 -->

    <owl:NamedIndividual rdf:about="http://purl.obolibrary.org/obo/GAZ_00266266">
        <obo:RO_0001025 rdf:resource="http://purl.obolibrary.org/obo/GAZ_00000508"/>
        <obo:IAO_0000115>A river.</obo:IAO_0000115>
        <oboInOwl:hasOBONamespace>GAZ</oboInOwl:hasOBONamespace>
        <oboInOwl:id>GAZ:00266266</oboInOwl:id>
        <rdfs:label>Rio Holmul</rdfs:label>
    </owl:NamedIndividual>
    


    <!-- http://purl.obolibrary.org/obo/GAZ_00266268 -->

    <owl:NamedIndividual rdf:about="http://purl.obolibrary.org/obo/GAZ_00266268">
        <obo:RO_0001025 rdf:resource="http://purl.obolibrary.org/obo/GAZ_00000508"/>
        <obo:IAO_0000115>A river.</obo:IAO_0000115>
        <oboInOwl:hasOBONamespace>GAZ</oboInOwl:hasOBONamespace>
        <oboInOwl:id>GAZ:00266268</oboInOwl:id>
        <rdfs:label>Rio Santa Amelia</rdfs:label>
    </owl:NamedIndividual>
    


    <!-- http://purl.obolibrary.org/obo/GAZ_00266269 -->

    <owl:NamedIndividual rdf:about="http://purl.obolibrary.org/obo/GAZ_00266269">
        <obo:RO_0001025 rdf:resource="http://purl.obolibrary.org/obo/GAZ_00000508"/>
        <obo:IAO_0000115>A river.</obo:IAO_0000115>
        <oboInOwl:hasOBONamespace>GAZ</oboInOwl:hasOBONamespace>
        <oboInOwl:id>GAZ:00266269</oboInOwl:id>
        <rdfs:label>Riachuelo Machaquila</rdfs:label>
    </owl:NamedIndividual>
    


    <!-- http://purl.obolibrary.org/obo/GAZ_00266270 -->

    <owl:NamedIndividual rdf:about="http://purl.obolibrary.org/obo/GAZ_00266270">
        <obo:RO_0001025 rdf:resource="http://purl.obolibrary.org/obo/GAZ_00000508"/>
        <obo:IAO_0000115>A river.</obo:IAO_0000115>
        <oboInOwl:hasOBONamespace>GAZ</oboInOwl:hasOBONamespace>
        <oboInOwl:id>GAZ:00266270</oboInOwl:id>
        <rdfs:label>Rio Poxte</rdfs:label>
    </owl:NamedIndividual>
    


    <!-- http://purl.obolibrary.org/obo/GAZ_00266271 -->

    <owl:NamedIndividual rdf:about="http://purl.obolibrary.org/obo/GAZ_00266271">
        <obo:RO_0001025 rdf:resource="http://purl.obolibrary.org/obo/GAZ_00000508"/>
        <obo:IAO_0000115>A river.</obo:IAO_0000115>
        <oboInOwl:hasOBONamespace>GAZ</oboInOwl:hasOBONamespace>
        <oboInOwl:id>GAZ:00266271</oboInOwl:id>
        <rdfs:label>Rio El Subin</rdfs:label>
    </owl:NamedIndividual>
    


    <!-- http://purl.obolibrary.org/obo/GAZ_00266273 -->

    <owl:NamedIndividual rdf:about="http://purl.obolibrary.org/obo/GAZ_00266273">
        <obo:RO_0001025 rdf:resource="http://purl.obolibrary.org/obo/GAZ_00000508"/>
        <obo:IAO_0000115>A river.</obo:IAO_0000115>
        <oboInOwl:hasOBONamespace>GAZ</oboInOwl:hasOBONamespace>
        <oboInOwl:id>GAZ:00266273</oboInOwl:id>
        <rdfs:label>Rio Chocop</rdfs:label>
    </owl:NamedIndividual>
    


    <!-- http://purl.obolibrary.org/obo/GAZ_00266274 -->

    <owl:NamedIndividual rdf:about="http://purl.obolibrary.org/obo/GAZ_00266274">
        <obo:RO_0001025 rdf:resource="http://purl.obolibrary.org/obo/GAZ_00000508"/>
        <obo:IAO_0000115>A river.</obo:IAO_0000115>
        <oboInOwl:hasOBONamespace>GAZ</oboInOwl:hasOBONamespace>
        <oboInOwl:id>GAZ:00266274</oboInOwl:id>
        <rdfs:label>Rio Xan</rdfs:label>
    </owl:NamedIndividual>
    


    <!-- http://purl.obolibrary.org/obo/GAZ_00266275 -->

    <owl:NamedIndividual rdf:about="http://purl.obolibrary.org/obo/GAZ_00266275">
        <obo:RO_0001025 rdf:resource="http://purl.obolibrary.org/obo/GAZ_00000508"/>
        <obo:IAO_0000115>A river.</obo:IAO_0000115>
        <oboInOwl:hasOBONamespace>GAZ</oboInOwl:hasOBONamespace>
        <oboInOwl:id>GAZ:00266275</oboInOwl:id>
        <rdfs:label>Rio San Juan</rdfs:label>
    </owl:NamedIndividual>
    


    <!-- http://purl.obolibrary.org/obo/GAZ_00266276 -->

    <owl:NamedIndividual rdf:about="http://purl.obolibrary.org/obo/GAZ_00266276">
        <obo:RO_0001025 rdf:resource="http://purl.obolibrary.org/obo/GAZ_00000508"/>
        <obo:IAO_0000115>A river.</obo:IAO_0000115>
        <oboInOwl:hasOBONamespace>GAZ</oboInOwl:hasOBONamespace>
        <oboInOwl:id>GAZ:00266276</oboInOwl:id>
        <rdfs:label>Arroyo Peje Lagarto</rdfs:label>
    </owl:NamedIndividual>
    


    <!-- http://purl.obolibrary.org/obo/GAZ_00266278 -->

    <owl:NamedIndividual rdf:about="http://purl.obolibrary.org/obo/GAZ_00266278">
        <obo:RO_0001025 rdf:resource="http://purl.obolibrary.org/obo/GAZ_00068206"/>
        <obo:IAO_0000115>A protected area. A forested hill overlooking the valley of Quetzaltenango. It is located at the south-eastern edge of the city of Quetzaltenango in Guatemala.</obo:IAO_0000115>
        <oboInOwl:hasOBONamespace>GAZ</oboInOwl:hasOBONamespace>
        <oboInOwl:id>GAZ:00266278</oboInOwl:id>
        <rdfs:label>Parque Nacional Cerro El Baul</rdfs:label>
    </owl:NamedIndividual>
    


    <!-- http://purl.obolibrary.org/obo/GAZ_00266279 -->

    <owl:NamedIndividual rdf:about="http://purl.obolibrary.org/obo/GAZ_00266279">
        <obo:RO_0001025 rdf:resource="http://purl.obolibrary.org/obo/GAZ_00068335"/>
        <obo:IAO_0000115>A protected area. A hill covered with dry shrubland located a few kilometers south of the city of Zacapa in Guatemala.</obo:IAO_0000115>
        <oboInOwl:hasOBONamespace>GAZ</oboInOwl:hasOBONamespace>
        <oboInOwl:id>GAZ:00266279</oboInOwl:id>
        <rdfs:label>Parque Nacional Cerro Miramundo</rdfs:label>
    </owl:NamedIndividual>
    


    <!-- http://purl.obolibrary.org/obo/GAZ_00266280 -->

    <owl:NamedIndividual rdf:about="http://purl.obolibrary.org/obo/GAZ_00266280">
        <obo:RO_0001025 rdf:resource="http://purl.obolibrary.org/obo/GAZ_00000476"/>
        <obo:IAO_0000115>A protected area. Established 1955.</obo:IAO_0000115>
        <oboInOwl:hasOBONamespace>GAZ</oboInOwl:hasOBONamespace>
        <oboInOwl:id>GAZ:00266280</oboInOwl:id>
        <rdfs:label>Parque Nacional Cerro El Reformador</rdfs:label>
    </owl:NamedIndividual>
    


    <!-- http://purl.obolibrary.org/obo/GAZ_00266281 -->

    <owl:NamedIndividual rdf:about="http://purl.obolibrary.org/obo/GAZ_00266281">
        <obo:RO_0001025 rdf:resource="http://purl.obolibrary.org/obo/GAZ_00068085"/>
        <obo:IAO_0000115>A protected area. A small forested park area with a number of springs and two small lakes. It is located a few kilometers south of the city of Chimaltenango in Guatemala. Established 1955.</obo:IAO_0000115>
        <oboInOwl:hasOBONamespace>GAZ</oboInOwl:hasOBONamespace>
        <oboInOwl:id>GAZ:00266281</oboInOwl:id>
        <rdfs:label>Parque Nacional Los Aposentos</rdfs:label>
    </owl:NamedIndividual>
    


    <!-- http://purl.obolibrary.org/obo/GAZ_00266282 -->

    <owl:NamedIndividual rdf:about="http://purl.obolibrary.org/obo/GAZ_00266282">
        <obo:RO_0001025 rdf:resource="http://purl.obolibrary.org/obo/GAZ_00005155"/>
        <obo:IAO_0000115>A protected area located 21 km south of Guatemala City, just north of Lake Amatitlan.</obo:IAO_0000115>
        <oboInOwl:hasOBONamespace>GAZ</oboInOwl:hasOBONamespace>
        <oboInOwl:id>GAZ:00266282</oboInOwl:id>
        <rdfs:label>Parque Nacional Naciones Unidas</rdfs:label>
    </owl:NamedIndividual>
    


    <!-- http://purl.obolibrary.org/obo/GAZ_00266283 -->

    <owl:NamedIndividual rdf:about="http://purl.obolibrary.org/obo/GAZ_00266283">
        <obo:RO_0001025 rdf:resource="http://purl.obolibrary.org/obo/GAZ_00068324"/>
        <obo:IAO_0000115>A protected area. Established 1955.</obo:IAO_0000115>
        <oboInOwl:hasOBONamespace>GAZ</oboInOwl:hasOBONamespace>
        <oboInOwl:id>GAZ:00266283</oboInOwl:id>
        <rdfs:label>Parque Nacional Riscos de Momostenango</rdfs:label>
    </owl:NamedIndividual>
    


    <!-- http://purl.obolibrary.org/obo/GAZ_00266284 -->

    <owl:NamedIndividual rdf:about="http://purl.obolibrary.org/obo/GAZ_00266284">
        <obo:RO_0001025 rdf:resource="http://purl.obolibrary.org/obo/GAZ_00000494"/>
        <obo:IAO_0000115>A protected area. Located along the banks of the Dulce river and the El Golfete.</obo:IAO_0000115>
        <oboInOwl:hasOBONamespace>GAZ</oboInOwl:hasOBONamespace>
        <oboInOwl:id>GAZ:00266284</oboInOwl:id>
        <rdfs:label>Parque Nacional Rio Dulce</rdfs:label>
    </owl:NamedIndividual>
    


    <!-- http://purl.obolibrary.org/obo/GAZ_00266285 -->

    <owl:NamedIndividual rdf:about="http://purl.obolibrary.org/obo/GAZ_00266285">
        <obo:RO_0001025 rdf:resource="http://purl.obolibrary.org/obo/GAZ_00068053"/>
        <obo:IAO_0000115>A protected area. Established 1976.</obo:IAO_0000115>
        <oboInOwl:hasOBONamespace>GAZ</oboInOwl:hasOBONamespace>
        <oboInOwl:id>GAZ:00266285</oboInOwl:id>
        <rdfs:label>Parque Nacional San Jose la Colonia</rdfs:label>
    </owl:NamedIndividual>
    


    <!-- http://purl.obolibrary.org/obo/GAZ_00266286 -->

    <owl:NamedIndividual rdf:about="http://purl.obolibrary.org/obo/GAZ_00266286">
        <obo:RO_0001025 rdf:resource="http://purl.obolibrary.org/obo/GAZ_00000494"/>
        <obo:IAO_0000115>A river in eastern Guatemala. Its sources are located on the eastern slopes of the Sierra de Santa Cruz. From there it flows in a generally west-south-west direction into the Golfete Dulce.</obo:IAO_0000115>
        <oboInOwl:hasOBONamespace>GAZ</oboInOwl:hasOBONamespace>
        <oboInOwl:id>GAZ:00266286</oboInOwl:id>
        <rdfs:label>Rio Chocon Machacas</rdfs:label>
    </owl:NamedIndividual>
    


    <!-- http://purl.obolibrary.org/obo/GAZ_00266733 -->

    <owl:NamedIndividual rdf:about="http://purl.obolibrary.org/obo/GAZ_00266733">
        <obo:IAO_0000115>A protected area. Established 1959-01-01.</obo:IAO_0000115>
        <oboInOwl:hasOBONamespace>GAZ</oboInOwl:hasOBONamespace>
        <oboInOwl:id>GAZ:00266733</oboInOwl:id>
        <rdfs:label>Parque Nacional El Cusuco</rdfs:label>
    </owl:NamedIndividual>
    


    <!-- http://purl.obolibrary.org/obo/GAZ_00266760 -->

    <owl:NamedIndividual rdf:about="http://purl.obolibrary.org/obo/GAZ_00266760">
        <obo:IAO_0000115>A river.</obo:IAO_0000115>
        <oboInOwl:hasOBONamespace>GAZ</oboInOwl:hasOBONamespace>
        <oboInOwl:id>GAZ:00266760</oboInOwl:id>
        <rdfs:label>Rio Guarajambala</rdfs:label>
    </owl:NamedIndividual>
    


    <!-- http://purl.obolibrary.org/obo/GAZ_00266761 -->

    <owl:NamedIndividual rdf:about="http://purl.obolibrary.org/obo/GAZ_00266761">
        <obo:IAO_0000115>A river.</obo:IAO_0000115>
        <oboInOwl:hasOBONamespace>GAZ</oboInOwl:hasOBONamespace>
        <oboInOwl:id>GAZ:00266761</oboInOwl:id>
        <rdfs:label>Rio Mocal</rdfs:label>
    </owl:NamedIndividual>
    


    <!-- 
    ///////////////////////////////////////////////////////////////////////////////////////
    //
    // Annotations
    //
    ///////////////////////////////////////////////////////////////////////////////////////
     -->

    <rdf:Description rdf:about="http://purl.obolibrary.org/obo/GAZ_00000430">
        <rdfs:label>Department of Alta Verapaz</rdfs:label>
        <obo:IAO_0000115>A department in the north central part of Guatemala. The capital and chief city of the department is Coban. Verapaz is bordered to the north by El Peten, to the east by Izabal, to the south by Zacapa, El Progreso, and Baja Verapaz, and to the west by El Quiche.</obo:IAO_0000115>
        <oboInOwl:hasOBONamespace>GAZ</oboInOwl:hasOBONamespace>
        <oboInOwl:id>GAZ:00000430</oboInOwl:id>
    </rdf:Description>
    <rdf:Description rdf:about="http://purl.obolibrary.org/obo/GAZ_00000433">
        <obo:IAO_0000115>A department in Guatemala. The capital is Salama.</obo:IAO_0000115>
        <rdfs:label>Department of Baja Verapaz</rdfs:label>
        <oboInOwl:hasOBONamespace>GAZ</oboInOwl:hasOBONamespace>
        <oboInOwl:id>GAZ:00000433</oboInOwl:id>
    </rdf:Description>
    <rdf:Description rdf:about="http://purl.obolibrary.org/obo/GAZ_00000439">
        <oboInOwl:hasOBONamespace>GAZ</oboInOwl:hasOBONamespace>
        <obo:IAO_0000115>A department of Guatemala. The capital is Chimaltenango.</obo:IAO_0000115>
        <oboInOwl:id>GAZ:00000439</oboInOwl:id>
        <rdfs:label>Department of Chimaltenango</rdfs:label>
    </rdf:Description>
    <rdf:Description rdf:about="http://purl.obolibrary.org/obo/GAZ_00000446">
        <oboInOwl:hasOBONamespace>GAZ</oboInOwl:hasOBONamespace>
        <obo:IAO_0000115>A department of Guatemala.</obo:IAO_0000115>
        <rdfs:label>Department of Chiquimula</rdfs:label>
        <oboInOwl:id>GAZ:00000446</oboInOwl:id>
    </rdf:Description>
    <rdf:Description rdf:about="http://purl.obolibrary.org/obo/GAZ_00000476">
        <oboInOwl:id>GAZ:00000476</oboInOwl:id>
        <oboInOwl:hasOBONamespace>GAZ</oboInOwl:hasOBONamespace>
        <obo:IAO_0000115>A department in Guatemala. The capital is Guastatoya and the largest city is Sanarate.</obo:IAO_0000115>
        <rdfs:label>Department of El Progreso</rdfs:label>
    </rdf:Description>
    <rdf:Description rdf:about="http://purl.obolibrary.org/obo/GAZ_00000477">
        <oboInOwl:id>GAZ:00000477</oboInOwl:id>
        <obo:IAO_0000115>One of the 22 departments of Guatemala. The capital is the city of Escuintla.</obo:IAO_0000115>
        <oboInOwl:hasOBONamespace>GAZ</oboInOwl:hasOBONamespace>
        <rdfs:label>Department of Escuintla</rdfs:label>
    </rdf:Description>
    <rdf:Description rdf:about="http://purl.obolibrary.org/obo/GAZ_00000483">
        <obo:IAO_0000115>One of the 22 departments of Guatemala. It bounds to the north with Mexico; to the east with Quiche, to the south with Totonicapan and San Marcos, and to the west again with Mexico. The capital is the city of Huehuetenango.</obo:IAO_0000115>
        <rdfs:label>Department of Huehuetenango</rdfs:label>
        <oboInOwl:hasOBONamespace>GAZ</oboInOwl:hasOBONamespace>
        <oboInOwl:id>GAZ:00000483</oboInOwl:id>
    </rdf:Description>
    <rdf:Description rdf:about="http://purl.obolibrary.org/obo/GAZ_00000494">
        <oboInOwl:hasOBONamespace>GAZ</oboInOwl:hasOBONamespace>
        <obo:IAO_0000115>One of the 22 departments of Guatemala. Izabal is bordered to the north by Belize, to the north east by the Gulf of Honduras, and to the east by Honduras, and by the Guatemalan departments of Peten to the north west, Alta Verapaz to the west, and Zacapa to the south.</obo:IAO_0000115>
        <rdfs:label>Department of Izabal</rdfs:label>
        <oboInOwl:id>GAZ:00000494</oboInOwl:id>
    </rdf:Description>
    <rdf:Description rdf:about="http://purl.obolibrary.org/obo/GAZ_00000496">
        <obo:IAO_0000115>A department of Guatemala, in the south east of the republic. The capital is the city of Jalapa.</obo:IAO_0000115>
        <oboInOwl:hasOBONamespace>GAZ</oboInOwl:hasOBONamespace>
        <oboInOwl:id>GAZ:00000496</oboInOwl:id>
        <rdfs:label>Department of Jalapa</rdfs:label>
    </rdf:Description>
    <rdf:Description rdf:about="http://purl.obolibrary.org/obo/GAZ_00000499">
        <oboInOwl:id>GAZ:00000499</oboInOwl:id>
        <oboInOwl:hasOBONamespace>GAZ</oboInOwl:hasOBONamespace>
        <rdfs:label>Department of Jutiapa</rdfs:label>
        <obo:IAO_0000115>A department of Guatemala that borders along El Salvador and the Pacific Ocean. The capital is the city of Jutiapa.</obo:IAO_0000115>
    </rdf:Description>
    <rdf:Description rdf:about="http://purl.obolibrary.org/obo/GAZ_00000508">
        <oboInOwl:id>GAZ:00000508</oboInOwl:id>
        <rdfs:label>Department of Peten</rdfs:label>
        <oboInOwl:hasOBONamespace>GAZ</oboInOwl:hasOBONamespace>
        <obo:IAO_0000115>A department of the nation of Guatemala.</obo:IAO_0000115>
    </rdf:Description>
    <rdf:Description rdf:about="http://purl.obolibrary.org/obo/GAZ_00000510">
        <obo:IAO_0000115>A department in Guatemala. The capital is the city of Quetzaltenango.</obo:IAO_0000115>
        <rdfs:label>Department of Quetzaltenango</rdfs:label>
        <oboInOwl:id>GAZ:00000510</oboInOwl:id>
        <oboInOwl:hasOBONamespace>GAZ</oboInOwl:hasOBONamespace>
    </rdf:Description>
    <rdf:Description rdf:about="http://purl.obolibrary.org/obo/GAZ_00000517">
        <oboInOwl:id>GAZ:00000517</oboInOwl:id>
        <rdfs:label>Department of Quiche</rdfs:label>
        <obo:IAO_0000115>A department of Guatemala. Located to the north-west of Guatemala City. The capital is Santa Cruz del Quiche.</obo:IAO_0000115>
        <oboInOwl:hasOBONamespace>GAZ</oboInOwl:hasOBONamespace>
    </rdf:Description>
    <rdf:Description rdf:about="http://purl.obolibrary.org/obo/GAZ_00000522">
        <obo:IAO_0000115>A department located in the south-west of Guatemala, extending from the mountains to the Pacific Ocean coast. The capital is the city of Retalhuleu.</obo:IAO_0000115>
        <rdfs:label>Department of Retalhuleu</rdfs:label>
        <oboInOwl:id>GAZ:00000522</oboInOwl:id>
        <oboInOwl:hasOBONamespace>GAZ</oboInOwl:hasOBONamespace>
    </rdf:Description>
    <rdf:Description rdf:about="http://purl.obolibrary.org/obo/GAZ_00000525">
        <rdfs:label>Department of Sacatepequez</rdfs:label>
        <obo:IAO_0000115>One of the 22 departments of Guatemala. The capital of Sacatepequez is Antigua Guatemala.</obo:IAO_0000115>
        <oboInOwl:id>GAZ:00000525</oboInOwl:id>
        <oboInOwl:hasOBONamespace>GAZ</oboInOwl:hasOBONamespace>
    </rdf:Description>
    <rdf:Description rdf:about="http://purl.obolibrary.org/obo/GAZ_00000529">
        <rdfs:label>Department of San Marcos</rdfs:label>
        <oboInOwl:id>GAZ:00000529</oboInOwl:id>
        <oboInOwl:hasOBONamespace>GAZ</oboInOwl:hasOBONamespace>
        <obo:IAO_0000115>A department in Guatemala. The capital is the city of San Marcos.</obo:IAO_0000115>
    </rdf:Description>
    <rdf:Description rdf:about="http://purl.obolibrary.org/obo/GAZ_00000540">
        <oboInOwl:id>GAZ:00000540</oboInOwl:id>
        <rdfs:label>Department of Santa Rosa</rdfs:label>
        <obo:IAO_0000115>A department in Guatemala. The capital is Cuilapa.</obo:IAO_0000115>
        <oboInOwl:hasOBONamespace>GAZ</oboInOwl:hasOBONamespace>
    </rdf:Description>
    <rdf:Description rdf:about="http://purl.obolibrary.org/obo/GAZ_00000541">
        <rdfs:label>Department of Solola</rdfs:label>
        <obo:IAO_0000115>A department in the west of Guatemala. The capital is the city of Solola.</obo:IAO_0000115>
        <oboInOwl:id>GAZ:00000541</oboInOwl:id>
        <oboInOwl:hasOBONamespace>GAZ</oboInOwl:hasOBONamespace>
    </rdf:Description>
    <rdf:Description rdf:about="http://purl.obolibrary.org/obo/GAZ_00000545">
        <rdfs:label>Department of Suchitepequez</rdfs:label>
        <oboInOwl:id>GAZ:00000545</oboInOwl:id>
        <obo:IAO_0000115>One of the 22 departments of Guatemala. The capital is Mazatenango. It is situated in the Southwestern region of Guatemala, bordered to the North by Quezaltenango, Solola and Chimaltenango; to the South by the Pacific Ocean; East byith Escuintla, and West by Retalhuleu.</obo:IAO_0000115>
        <oboInOwl:hasOBONamespace>GAZ</oboInOwl:hasOBONamespace>
    </rdf:Description>
    <rdf:Description rdf:about="http://purl.obolibrary.org/obo/GAZ_00000548">
        <oboInOwl:hasOBONamespace>GAZ</oboInOwl:hasOBONamespace>
        <obo:IAO_0000115>One of the 22 departments of Guatemala. The capital is the city of Zacapa.</obo:IAO_0000115>
        <oboInOwl:id>GAZ:00000548</oboInOwl:id>
        <rdfs:label>Department of Zacapa</rdfs:label>
    </rdf:Description>
    <rdf:Description rdf:about="http://purl.obolibrary.org/obo/GAZ_00000549">
        <oboInOwl:hasOBONamespace>GAZ</oboInOwl:hasOBONamespace>
        <obo:IAO_0000115>One of the 22 departments of Guatemala. The capital is the city of Totonicapan.</obo:IAO_0000115>
        <oboInOwl:id>GAZ:00000549</oboInOwl:id>
        <rdfs:label>Department of Totonicapan</rdfs:label>
    </rdf:Description>
    <rdf:Description rdf:about="http://purl.obolibrary.org/obo/GAZ_00005152">
        <oboInOwl:id>GAZ:00005152</oboInOwl:id>
        <oboInOwl:hasOBONamespace>GAZ</oboInOwl:hasOBONamespace>
        <rdfs:label>Department (Guatemala)</rdfs:label>
    </rdf:Description>
    <rdf:Description rdf:about="http://purl.obolibrary.org/obo/GAZ_00005153">
        <oboInOwl:id>GAZ:00005153</oboInOwl:id>
        <oboInOwl:hasOBONamespace>GAZ</oboInOwl:hasOBONamespace>
        <rdfs:label>populated place, Guatemala</rdfs:label>
    </rdf:Description>
    <rdf:Description rdf:about="http://purl.obolibrary.org/obo/GAZ_00005154">
        <rdfs:label>Guatemala City</rdfs:label>
        <oboInOwl:hasOBONamespace>GAZ</oboInOwl:hasOBONamespace>
        <oboInOwl:id>GAZ:00005154</oboInOwl:id>
        <obo:IAO_0000115>The capital and largest city of the Republic of Guatemala.</obo:IAO_0000115>
    </rdf:Description>
    <rdf:Description rdf:about="http://purl.obolibrary.org/obo/GAZ_00005155">
        <oboInOwl:hasOBONamespace>GAZ</oboInOwl:hasOBONamespace>
        <obo:IAO_0000115>One of the 22 departments of Guatemala. The capital is Guatemala City, which also serves as the national capital.</obo:IAO_0000115>
        <rdfs:label>Department of Guatemala</rdfs:label>
        <oboInOwl:id>GAZ:00005155</oboInOwl:id>
    </rdf:Description>
    <rdf:Description rdf:about="http://purl.obolibrary.org/obo/GAZ_00056113">
        <oboInOwl:id>GAZ:00056113</oboInOwl:id>
        <rdfs:label>Panajachel</rdfs:label>
        <obo:IAO_0000115>A populated place. A town in the southwestern Guatemalan Highlands, in the department of Solola.</obo:IAO_0000115>
        <oboInOwl:hasOBONamespace>GAZ</oboInOwl:hasOBONamespace>
    </rdf:Description>
</rdf:RDF>



<!-- Generated by the OWL API (version 4.5.6) https://github.com/owlcs/owlapi -->

