<?xml version="1.0"?>
<rdf:RDF xmlns="http://purl.obolibrary.org/obo/gaz/subsets/countries/Hungary.owl#"
     xml:base="http://purl.obolibrary.org/obo/gaz/subsets/countries/Hungary.owl"
     xmlns:obo="http://purl.obolibrary.org/obo/"
     xmlns:owl="http://www.w3.org/2002/07/owl#"
     xmlns:rdf="http://www.w3.org/1999/02/22-rdf-syntax-ns#"
     xmlns:xml="http://www.w3.org/XML/1998/namespace"
     xmlns:xsd="http://www.w3.org/2001/XMLSchema#"
     xmlns:rdfs="http://www.w3.org/2000/01/rdf-schema#"
     xmlns:oboInOwl="http://www.geneontology.org/formats/oboInOwl#">
    <owl:Ontology rdf:about="http://purl.obolibrary.org/obo/gaz/subsets/countries/Hungary.owl">
        <owl:imports rdf:resource="http://purl.obolibrary.org/obo/gaz/imports/envo_import.owl"/>
        <owl:imports rdf:resource="http://purl.obolibrary.org/obo/gaz/imports/ro_import.owl"/>
    </owl:Ontology>
    


    <!-- 
    ///////////////////////////////////////////////////////////////////////////////////////
    //
    // Annotation properties
    //
    ///////////////////////////////////////////////////////////////////////////////////////
     -->

    


    <!-- http://purl.obolibrary.org/obo/IAO_0000115 -->

    <owl:AnnotationProperty rdf:about="http://purl.obolibrary.org/obo/IAO_0000115"/>
    


    <!-- http://www.geneontology.org/formats/oboInOwl#hasOBONamespace -->

    <owl:AnnotationProperty rdf:about="http://www.geneontology.org/formats/oboInOwl#hasOBONamespace"/>
    


    <!-- http://www.geneontology.org/formats/oboInOwl#id -->

    <owl:AnnotationProperty rdf:about="http://www.geneontology.org/formats/oboInOwl#id"/>
    


    <!-- 
    ///////////////////////////////////////////////////////////////////////////////////////
    //
    // Object Properties
    //
    ///////////////////////////////////////////////////////////////////////////////////////
     -->

    


    <!-- http://purl.obolibrary.org/obo/RO_0001025 -->

    <owl:ObjectProperty rdf:about="http://purl.obolibrary.org/obo/RO_0001025"/>
    


    <!-- 
    ///////////////////////////////////////////////////////////////////////////////////////
    //
    // Classes
    //
    ///////////////////////////////////////////////////////////////////////////////////////
     -->

    


    <!-- http://purl.obolibrary.org/obo/ENVO_00000080 -->

    <owl:Class rdf:about="http://purl.obolibrary.org/obo/ENVO_00000080"/>
    


    <!-- http://purl.obolibrary.org/obo/ENVO_00000100 -->

    <owl:Class rdf:about="http://purl.obolibrary.org/obo/ENVO_00000100"/>
    


    <!-- http://purl.obolibrary.org/obo/ENVO_00000104 -->

    <owl:Class rdf:about="http://purl.obolibrary.org/obo/ENVO_00000104"/>
    


    <!-- http://purl.obolibrary.org/obo/ENVO_00000106 -->

    <owl:Class rdf:about="http://purl.obolibrary.org/obo/ENVO_00000106"/>
    


    <!-- http://purl.obolibrary.org/obo/ENVO_00000423 -->

    <owl:Class rdf:about="http://purl.obolibrary.org/obo/ENVO_00000423"/>
    


    <!-- http://purl.obolibrary.org/obo/ENVO_00000856 -->

    <owl:Class rdf:about="http://purl.obolibrary.org/obo/ENVO_00000856"/>
    


    <!-- http://purl.obolibrary.org/obo/GAZ_00003594 -->

    <owl:Class rdf:about="http://purl.obolibrary.org/obo/GAZ_00003594"/>
    


    <!-- http://purl.obolibrary.org/obo/GAZ_00003595 -->

    <owl:Class rdf:about="http://purl.obolibrary.org/obo/GAZ_00003595">
        <rdfs:subClassOf rdf:resource="http://purl.obolibrary.org/obo/GAZ_00003594"/>
    </owl:Class>
    


    <!-- http://purl.obolibrary.org/obo/GAZ_00003596 -->

    <owl:Class rdf:about="http://purl.obolibrary.org/obo/GAZ_00003596">
        <rdfs:subClassOf rdf:resource="http://purl.obolibrary.org/obo/GAZ_00003594"/>
    </owl:Class>
    


    <!-- http://purl.obolibrary.org/obo/GAZ_00003597 -->

    <owl:Class rdf:about="http://purl.obolibrary.org/obo/GAZ_00003597">
        <rdfs:subClassOf rdf:resource="http://purl.obolibrary.org/obo/GAZ_00003594"/>
    </owl:Class>
    


    <!-- http://purl.obolibrary.org/obo/GAZ_00003598 -->

    <owl:Class rdf:about="http://purl.obolibrary.org/obo/GAZ_00003598">
        <rdfs:subClassOf rdf:resource="http://purl.obolibrary.org/obo/GAZ_00003594"/>
    </owl:Class>
    


    <!-- http://purl.obolibrary.org/obo/GAZ_00003599 -->

    <owl:Class rdf:about="http://purl.obolibrary.org/obo/GAZ_00003599">
        <rdfs:subClassOf rdf:resource="http://purl.obolibrary.org/obo/GAZ_00003594"/>
    </owl:Class>
    


    <!-- http://purl.obolibrary.org/obo/GAZ_00003600 -->

    <owl:Class rdf:about="http://purl.obolibrary.org/obo/GAZ_00003600">
        <rdfs:subClassOf rdf:resource="http://purl.obolibrary.org/obo/GAZ_00003594"/>
    </owl:Class>
    


    <!-- http://purl.obolibrary.org/obo/GAZ_00003601 -->

    <owl:Class rdf:about="http://purl.obolibrary.org/obo/GAZ_00003601">
        <rdfs:subClassOf rdf:resource="http://purl.obolibrary.org/obo/GAZ_00003594"/>
    </owl:Class>
    


    <!-- http://purl.obolibrary.org/obo/GAZ_00003602 -->

    <owl:Class rdf:about="http://purl.obolibrary.org/obo/GAZ_00003602">
        <rdfs:subClassOf rdf:resource="http://purl.obolibrary.org/obo/GAZ_00003603"/>
    </owl:Class>
    


    <!-- http://purl.obolibrary.org/obo/GAZ_00003603 -->

    <owl:Class rdf:about="http://purl.obolibrary.org/obo/GAZ_00003603"/>
    


    <!-- http://purl.obolibrary.org/obo/GAZ_00004702 -->

    <owl:Class rdf:about="http://purl.obolibrary.org/obo/GAZ_00004702">
        <rdfs:subClassOf rdf:resource="http://purl.obolibrary.org/obo/GAZ_00003603"/>
    </owl:Class>
    


    <!-- http://purl.obolibrary.org/obo/GAZ_00008479 -->

    <owl:Class rdf:about="http://purl.obolibrary.org/obo/GAZ_00008479">
        <rdfs:subClassOf rdf:resource="http://purl.obolibrary.org/obo/GAZ_00003603"/>
    </owl:Class>
    


    <!-- http://purl.obolibrary.org/obo/GAZ_00010080 -->

    <owl:Class rdf:about="http://purl.obolibrary.org/obo/GAZ_00010080">
        <rdfs:subClassOf rdf:resource="http://purl.obolibrary.org/obo/GAZ_00003603"/>
    </owl:Class>
    


    <!-- http://purl.obolibrary.org/obo/GAZ_00036861 -->

    <owl:Class rdf:about="http://purl.obolibrary.org/obo/GAZ_00036861">
        <rdfs:subClassOf rdf:resource="http://purl.obolibrary.org/obo/GAZ_00003603"/>
    </owl:Class>
    


    <!-- http://purl.obolibrary.org/obo/GAZ_00043965 -->

    <owl:Class rdf:about="http://purl.obolibrary.org/obo/GAZ_00043965">
        <rdfs:subClassOf rdf:resource="http://purl.obolibrary.org/obo/GAZ_00003603"/>
    </owl:Class>
    


    <!-- http://purl.obolibrary.org/obo/GAZ_00103879 -->

    <owl:Class rdf:about="http://purl.obolibrary.org/obo/GAZ_00103879">
        <rdfs:subClassOf rdf:resource="http://purl.obolibrary.org/obo/GAZ_00003603"/>
    </owl:Class>
    


    <!-- http://purl.obolibrary.org/obo/GAZ_00148095 -->

    <owl:Class rdf:about="http://purl.obolibrary.org/obo/GAZ_00148095"/>
    


    <!-- http://purl.obolibrary.org/obo/GAZ_00148096 -->

    <owl:Class rdf:about="http://purl.obolibrary.org/obo/GAZ_00148096">
        <rdfs:subClassOf rdf:resource="http://purl.obolibrary.org/obo/GAZ_00148095"/>
    </owl:Class>
    


    <!-- http://purl.obolibrary.org/obo/GAZ_00148097 -->

    <owl:Class rdf:about="http://purl.obolibrary.org/obo/GAZ_00148097">
        <rdfs:subClassOf rdf:resource="http://purl.obolibrary.org/obo/GAZ_00148095"/>
    </owl:Class>
    


    <!-- http://purl.obolibrary.org/obo/GAZ_00148098 -->

    <owl:Class rdf:about="http://purl.obolibrary.org/obo/GAZ_00148098">
        <rdfs:subClassOf rdf:resource="http://purl.obolibrary.org/obo/GAZ_00148095"/>
    </owl:Class>
    


    <!-- http://purl.obolibrary.org/obo/GAZ_00148099 -->

    <owl:Class rdf:about="http://purl.obolibrary.org/obo/GAZ_00148099">
        <rdfs:subClassOf rdf:resource="http://purl.obolibrary.org/obo/GAZ_00148095"/>
    </owl:Class>
    


    <!-- http://purl.obolibrary.org/obo/GAZ_00148100 -->

    <owl:Class rdf:about="http://purl.obolibrary.org/obo/GAZ_00148100">
        <rdfs:subClassOf rdf:resource="http://purl.obolibrary.org/obo/GAZ_00148095"/>
    </owl:Class>
    


    <!-- http://purl.obolibrary.org/obo/GAZ_00148101 -->

    <owl:Class rdf:about="http://purl.obolibrary.org/obo/GAZ_00148101">
        <rdfs:subClassOf rdf:resource="http://purl.obolibrary.org/obo/GAZ_00148095"/>
    </owl:Class>
    


    <!-- http://purl.obolibrary.org/obo/GAZ_00148102 -->

    <owl:Class rdf:about="http://purl.obolibrary.org/obo/GAZ_00148102">
        <rdfs:subClassOf rdf:resource="http://purl.obolibrary.org/obo/GAZ_00148095"/>
    </owl:Class>
    


    <!-- http://purl.obolibrary.org/obo/GAZ_00148103 -->

    <owl:Class rdf:about="http://purl.obolibrary.org/obo/GAZ_00148103">
        <rdfs:subClassOf rdf:resource="http://purl.obolibrary.org/obo/GAZ_00148095"/>
    </owl:Class>
    


    <!-- http://purl.obolibrary.org/obo/GAZ_00148104 -->

    <owl:Class rdf:about="http://purl.obolibrary.org/obo/GAZ_00148104">
        <rdfs:subClassOf rdf:resource="http://purl.obolibrary.org/obo/GAZ_00148095"/>
    </owl:Class>
    


    <!-- http://purl.obolibrary.org/obo/GAZ_00148105 -->

    <owl:Class rdf:about="http://purl.obolibrary.org/obo/GAZ_00148105">
        <rdfs:subClassOf rdf:resource="http://purl.obolibrary.org/obo/GAZ_00148095"/>
    </owl:Class>
    


    <!-- http://purl.obolibrary.org/obo/GAZ_00148106 -->

    <owl:Class rdf:about="http://purl.obolibrary.org/obo/GAZ_00148106">
        <rdfs:subClassOf rdf:resource="http://purl.obolibrary.org/obo/GAZ_00148095"/>
    </owl:Class>
    


    <!-- http://purl.obolibrary.org/obo/GAZ_00148107 -->

    <owl:Class rdf:about="http://purl.obolibrary.org/obo/GAZ_00148107">
        <rdfs:subClassOf rdf:resource="http://purl.obolibrary.org/obo/GAZ_00148095"/>
    </owl:Class>
    


    <!-- http://purl.obolibrary.org/obo/GAZ_00148108 -->

    <owl:Class rdf:about="http://purl.obolibrary.org/obo/GAZ_00148108">
        <rdfs:subClassOf rdf:resource="http://purl.obolibrary.org/obo/GAZ_00148095"/>
    </owl:Class>
    


    <!-- http://purl.obolibrary.org/obo/GAZ_00148109 -->

    <owl:Class rdf:about="http://purl.obolibrary.org/obo/GAZ_00148109">
        <rdfs:subClassOf rdf:resource="http://purl.obolibrary.org/obo/GAZ_00148095"/>
    </owl:Class>
    


    <!-- http://purl.obolibrary.org/obo/GAZ_00148110 -->

    <owl:Class rdf:about="http://purl.obolibrary.org/obo/GAZ_00148110">
        <rdfs:subClassOf rdf:resource="http://purl.obolibrary.org/obo/GAZ_00148095"/>
    </owl:Class>
    


    <!-- http://purl.obolibrary.org/obo/GAZ_00148111 -->

    <owl:Class rdf:about="http://purl.obolibrary.org/obo/GAZ_00148111">
        <rdfs:subClassOf rdf:resource="http://purl.obolibrary.org/obo/GAZ_00148095"/>
    </owl:Class>
    


    <!-- http://purl.obolibrary.org/obo/GAZ_00148112 -->

    <owl:Class rdf:about="http://purl.obolibrary.org/obo/GAZ_00148112">
        <rdfs:subClassOf rdf:resource="http://purl.obolibrary.org/obo/GAZ_00148095"/>
    </owl:Class>
    


    <!-- http://purl.obolibrary.org/obo/GAZ_00148113 -->

    <owl:Class rdf:about="http://purl.obolibrary.org/obo/GAZ_00148113">
        <rdfs:subClassOf rdf:resource="http://purl.obolibrary.org/obo/GAZ_00148095"/>
    </owl:Class>
    


    <!-- http://purl.obolibrary.org/obo/GAZ_00148114 -->

    <owl:Class rdf:about="http://purl.obolibrary.org/obo/GAZ_00148114">
        <rdfs:subClassOf rdf:resource="http://purl.obolibrary.org/obo/GAZ_00148095"/>
    </owl:Class>
    


    <!-- http://purl.obolibrary.org/obo/GAZ_00148115 -->

    <owl:Class rdf:about="http://purl.obolibrary.org/obo/GAZ_00148115">
        <rdfs:subClassOf rdf:resource="http://purl.obolibrary.org/obo/GAZ_00148095"/>
    </owl:Class>
    


    <!-- http://purl.obolibrary.org/obo/GAZ_00148117 -->

    <owl:Class rdf:about="http://purl.obolibrary.org/obo/GAZ_00148117">
        <rdfs:subClassOf rdf:resource="http://purl.obolibrary.org/obo/GAZ_00148095"/>
    </owl:Class>
    


    <!-- http://purl.obolibrary.org/obo/GAZ_00148118 -->

    <owl:Class rdf:about="http://purl.obolibrary.org/obo/GAZ_00148118">
        <rdfs:subClassOf rdf:resource="http://purl.obolibrary.org/obo/GAZ_00148095"/>
    </owl:Class>
    


    <!-- http://purl.obolibrary.org/obo/GAZ_00148119 -->

    <owl:Class rdf:about="http://purl.obolibrary.org/obo/GAZ_00148119">
        <rdfs:subClassOf rdf:resource="http://purl.obolibrary.org/obo/GAZ_00148095"/>
    </owl:Class>
    


    <!-- http://purl.obolibrary.org/obo/GAZ_00148120 -->

    <owl:Class rdf:about="http://purl.obolibrary.org/obo/GAZ_00148120">
        <rdfs:subClassOf rdf:resource="http://purl.obolibrary.org/obo/GAZ_00148095"/>
    </owl:Class>
    


    <!-- http://purl.obolibrary.org/obo/GAZ_00148563 -->

    <owl:Class rdf:about="http://purl.obolibrary.org/obo/GAZ_00148563"/>
    


    <!-- http://purl.obolibrary.org/obo/GAZ_00481281 -->

    <owl:Class rdf:about="http://purl.obolibrary.org/obo/GAZ_00481281"/>
    


    <!-- http://purl.obolibrary.org/obo/GAZ_00481282 -->

    <owl:Class rdf:about="http://purl.obolibrary.org/obo/GAZ_00481282">
        <rdfs:subClassOf rdf:resource="http://purl.obolibrary.org/obo/GAZ_00481281"/>
        <obo:IAO_0000115>A lake.</obo:IAO_0000115>
        <oboInOwl:hasOBONamespace>GAZ</oboInOwl:hasOBONamespace>
        <oboInOwl:id>GAZ:00481282</oboInOwl:id>
        <rdfs:label>Vysne Rachkovo pleso</rdfs:label>
    </owl:Class>
    


    <!-- http://purl.obolibrary.org/obo/GAZ_00607653 -->

    <owl:Class rdf:about="http://purl.obolibrary.org/obo/GAZ_00607653">
        <obo:IAO_0000115>A river.</obo:IAO_0000115>
        <oboInOwl:hasOBONamespace>GAZ</oboInOwl:hasOBONamespace>
        <oboInOwl:id>GAZ:00607653</oboInOwl:id>
        <rdfs:label>Schwabinger Bach</rdfs:label>
    </owl:Class>
    


    <!-- http://purl.obolibrary.org/obo/GAZ_00607654 -->

    <owl:Class rdf:about="http://purl.obolibrary.org/obo/GAZ_00607654">
        <obo:IAO_0000115>A river.</obo:IAO_0000115>
        <oboInOwl:hasOBONamespace>GAZ</oboInOwl:hasOBONamespace>
        <oboInOwl:id>GAZ:00607654</oboInOwl:id>
        <rdfs:label>Eisbach</rdfs:label>
    </owl:Class>
    


    <!-- http://purl.obolibrary.org/obo/GAZ_00619830 -->

    <owl:Class rdf:about="http://purl.obolibrary.org/obo/GAZ_00619830"/>
    


    <!-- http://purl.obolibrary.org/obo/GAZ_00619831 -->

    <owl:Class rdf:about="http://purl.obolibrary.org/obo/GAZ_00619831">
        <obo:IAO_0000115>A river.</obo:IAO_0000115>
        <oboInOwl:hasOBONamespace>GAZ</oboInOwl:hasOBONamespace>
        <oboInOwl:id>GAZ:00619831</oboInOwl:id>
        <rdfs:label>Dreimuhlenbch</rdfs:label>
    </owl:Class>
    


    <!-- http://purl.obolibrary.org/obo/GAZ_00619832 -->

    <owl:Class rdf:about="http://purl.obolibrary.org/obo/GAZ_00619832">
        <obo:IAO_0000115>A river.</obo:IAO_0000115>
        <oboInOwl:hasOBONamespace>GAZ</oboInOwl:hasOBONamespace>
        <oboInOwl:id>GAZ:00619832</oboInOwl:id>
        <rdfs:label>Grosser Stadtbach</rdfs:label>
    </owl:Class>
    


    <!-- http://purl.obolibrary.org/obo/GAZ_00619833 -->

    <owl:Class rdf:about="http://purl.obolibrary.org/obo/GAZ_00619833">
        <obo:IAO_0000115>A river.</obo:IAO_0000115>
        <oboInOwl:hasOBONamespace>GAZ</oboInOwl:hasOBONamespace>
        <oboInOwl:id>GAZ:00619833</oboInOwl:id>
        <rdfs:label>Westmuhlbach</rdfs:label>
    </owl:Class>
    


    <!-- http://purl.obolibrary.org/obo/GAZ_00619834 -->

    <owl:Class rdf:about="http://purl.obolibrary.org/obo/GAZ_00619834">
        <obo:IAO_0000115>A river.</obo:IAO_0000115>
        <oboInOwl:hasOBONamespace>GAZ</oboInOwl:hasOBONamespace>
        <oboInOwl:id>GAZ:00619834</oboInOwl:id>
        <rdfs:label>Pesenbach</rdfs:label>
    </owl:Class>
    


    <!-- http://purl.obolibrary.org/obo/GAZ_00619835 -->

    <owl:Class rdf:about="http://purl.obolibrary.org/obo/GAZ_00619835">
        <obo:IAO_0000115>A river.</obo:IAO_0000115>
        <oboInOwl:hasOBONamespace>GAZ</oboInOwl:hasOBONamespace>
        <oboInOwl:id>GAZ:00619835</oboInOwl:id>
        <rdfs:label>Bleicherbachl</rdfs:label>
    </owl:Class>
    


    <!-- http://purl.obolibrary.org/obo/GAZ_00619836 -->

    <owl:Class rdf:about="http://purl.obolibrary.org/obo/GAZ_00619836">
        <obo:IAO_0000115>A river.</obo:IAO_0000115>
        <oboInOwl:hasOBONamespace>GAZ</oboInOwl:hasOBONamespace>
        <oboInOwl:id>GAZ:00619836</oboInOwl:id>
        <rdfs:label>Blererbachl</rdfs:label>
    </owl:Class>
    


    <!-- http://purl.obolibrary.org/obo/GAZ_00619837 -->

    <owl:Class rdf:about="http://purl.obolibrary.org/obo/GAZ_00619837">
        <obo:IAO_0000115>A river.</obo:IAO_0000115>
        <oboInOwl:hasOBONamespace>GAZ</oboInOwl:hasOBONamespace>
        <oboInOwl:id>GAZ:00619837</oboInOwl:id>
        <rdfs:label>Glockenbach</rdfs:label>
    </owl:Class>
    


    <!-- http://purl.obolibrary.org/obo/GAZ_00619838 -->

    <owl:Class rdf:about="http://purl.obolibrary.org/obo/GAZ_00619838">
        <obo:IAO_0000115>A river.</obo:IAO_0000115>
        <oboInOwl:hasOBONamespace>GAZ</oboInOwl:hasOBONamespace>
        <oboInOwl:id>GAZ:00619838</oboInOwl:id>
        <rdfs:label>Mahlmuhlbach</rdfs:label>
    </owl:Class>
    


    <!-- http://purl.obolibrary.org/obo/GAZ_00619839 -->

    <owl:Class rdf:about="http://purl.obolibrary.org/obo/GAZ_00619839">
        <obo:IAO_0000115>A river.</obo:IAO_0000115>
        <oboInOwl:hasOBONamespace>GAZ</oboInOwl:hasOBONamespace>
        <oboInOwl:id>GAZ:00619839</oboInOwl:id>
        <rdfs:label>Gipsmuhlkanak</rdfs:label>
    </owl:Class>
    


    <!-- http://purl.obolibrary.org/obo/GAZ_00619840 -->

    <owl:Class rdf:about="http://purl.obolibrary.org/obo/GAZ_00619840">
        <obo:IAO_0000115>A river.</obo:IAO_0000115>
        <oboInOwl:hasOBONamespace>GAZ</oboInOwl:hasOBONamespace>
        <oboInOwl:id>GAZ:00619840</oboInOwl:id>
        <rdfs:label>Grosser Angerbach</rdfs:label>
    </owl:Class>
    


    <!-- http://purl.obolibrary.org/obo/GAZ_00619841 -->

    <owl:Class rdf:about="http://purl.obolibrary.org/obo/GAZ_00619841">
        <obo:IAO_0000115>A river.</obo:IAO_0000115>
        <oboInOwl:hasOBONamespace>GAZ</oboInOwl:hasOBONamespace>
        <oboInOwl:id>GAZ:00619841</oboInOwl:id>
        <rdfs:label>Kleiner Angerbach</rdfs:label>
    </owl:Class>
    


    <!-- http://purl.obolibrary.org/obo/GAZ_00619842 -->

    <owl:Class rdf:about="http://purl.obolibrary.org/obo/GAZ_00619842">
        <obo:IAO_0000115>A river.</obo:IAO_0000115>
        <oboInOwl:hasOBONamespace>GAZ</oboInOwl:hasOBONamespace>
        <oboInOwl:id>GAZ:00619842</oboInOwl:id>
        <rdfs:label>Fabrikbach</rdfs:label>
    </owl:Class>
    


    <!-- http://purl.obolibrary.org/obo/GAZ_00619843 -->

    <owl:Class rdf:about="http://purl.obolibrary.org/obo/GAZ_00619843">
        <obo:IAO_0000115>A river.</obo:IAO_0000115>
        <oboInOwl:hasOBONamespace>GAZ</oboInOwl:hasOBONamespace>
        <oboInOwl:id>GAZ:00619843</oboInOwl:id>
        <rdfs:label>Apothekerbachl</rdfs:label>
    </owl:Class>
    


    <!-- http://purl.obolibrary.org/obo/GAZ_00619844 -->

    <owl:Class rdf:about="http://purl.obolibrary.org/obo/GAZ_00619844">
        <obo:IAO_0000115>A river.</obo:IAO_0000115>
        <oboInOwl:hasOBONamespace>GAZ</oboInOwl:hasOBONamespace>
        <oboInOwl:id>GAZ:00619844</oboInOwl:id>
        <rdfs:label>Einschuttbach</rdfs:label>
    </owl:Class>
    


    <!-- http://purl.obolibrary.org/obo/GAZ_00619845 -->

    <owl:Class rdf:about="http://purl.obolibrary.org/obo/GAZ_00619845">
        <obo:IAO_0000115>A river.</obo:IAO_0000115>
        <oboInOwl:hasOBONamespace>GAZ</oboInOwl:hasOBONamespace>
        <oboInOwl:id>GAZ:00619845</oboInOwl:id>
        <rdfs:label>Farbergrabenbach</rdfs:label>
    </owl:Class>
    


    <!-- http://purl.obolibrary.org/obo/GAZ_00619847 -->

    <owl:Class rdf:about="http://purl.obolibrary.org/obo/GAZ_00619847">
        <obo:IAO_0000115>A river.</obo:IAO_0000115>
        <oboInOwl:hasOBONamespace>GAZ</oboInOwl:hasOBONamespace>
        <oboInOwl:id>GAZ:00619847</oboInOwl:id>
        <rdfs:label>Holzartenkanal</rdfs:label>
    </owl:Class>
    


    <!-- http://purl.obolibrary.org/obo/GAZ_00619848 -->

    <owl:Class rdf:about="http://purl.obolibrary.org/obo/GAZ_00619848">
        <obo:IAO_0000115>A river.</obo:IAO_0000115>
        <oboInOwl:hasOBONamespace>GAZ</oboInOwl:hasOBONamespace>
        <oboInOwl:id>GAZ:00619848</oboInOwl:id>
        <rdfs:label>Eiener Kanal</rdfs:label>
    </owl:Class>
    


    <!-- http://purl.obolibrary.org/obo/GAZ_00619849 -->

    <owl:Class rdf:about="http://purl.obolibrary.org/obo/GAZ_00619849">
        <obo:IAO_0000115>A river.</obo:IAO_0000115>
        <oboInOwl:hasOBONamespace>GAZ</oboInOwl:hasOBONamespace>
        <oboInOwl:id>GAZ:00619849</oboInOwl:id>
        <rdfs:label>Brauhausbachl</rdfs:label>
    </owl:Class>
    


    <!-- http://purl.obolibrary.org/obo/GAZ_00619850 -->

    <owl:Class rdf:about="http://purl.obolibrary.org/obo/GAZ_00619850">
        <obo:IAO_0000115>A river.</obo:IAO_0000115>
        <oboInOwl:hasOBONamespace>GAZ</oboInOwl:hasOBONamespace>
        <oboInOwl:id>GAZ:00619850</oboInOwl:id>
        <rdfs:label>Ostlicher Stadtgrabenbach</rdfs:label>
    </owl:Class>
    


    <!-- http://purl.obolibrary.org/obo/GAZ_00619851 -->

    <owl:Class rdf:about="http://purl.obolibrary.org/obo/GAZ_00619851">
        <obo:IAO_0000115>A river.</obo:IAO_0000115>
        <oboInOwl:hasOBONamespace>GAZ</oboInOwl:hasOBONamespace>
        <oboInOwl:id>GAZ:00619851</oboInOwl:id>
        <rdfs:label>Westlicher Stadtgrabekbach</rdfs:label>
    </owl:Class>
    


    <!-- http://purl.obolibrary.org/obo/GAZ_00619852 -->

    <owl:Class rdf:about="http://purl.obolibrary.org/obo/GAZ_00619852">
        <obo:IAO_0000115>A river.</obo:IAO_0000115>
        <oboInOwl:hasOBONamespace>GAZ</oboInOwl:hasOBONamespace>
        <oboInOwl:id>GAZ:00619852</oboInOwl:id>
        <rdfs:label>Feuerbachl</rdfs:label>
    </owl:Class>
    


    <!-- http://purl.obolibrary.org/obo/GAZ_00619853 -->

    <owl:Class rdf:about="http://purl.obolibrary.org/obo/GAZ_00619853">
        <obo:IAO_0000115>A river.</obo:IAO_0000115>
        <oboInOwl:hasOBONamespace>GAZ</oboInOwl:hasOBONamespace>
        <oboInOwl:id>GAZ:00619853</oboInOwl:id>
        <rdfs:label>Feuerhausbachl</rdfs:label>
    </owl:Class>
    


    <!-- http://purl.obolibrary.org/obo/GAZ_00619854 -->

    <owl:Class rdf:about="http://purl.obolibrary.org/obo/GAZ_00619854">
        <obo:IAO_0000115>A river.</obo:IAO_0000115>
        <oboInOwl:hasOBONamespace>GAZ</oboInOwl:hasOBONamespace>
        <oboInOwl:id>GAZ:00619854</oboInOwl:id>
        <rdfs:label>Fischerbach</rdfs:label>
    </owl:Class>
    


    <!-- http://purl.obolibrary.org/obo/GAZ_00619856 -->

    <owl:Class rdf:about="http://purl.obolibrary.org/obo/GAZ_00619856">
        <obo:IAO_0000115>A river.</obo:IAO_0000115>
        <oboInOwl:hasOBONamespace>GAZ</oboInOwl:hasOBONamespace>
        <oboInOwl:id>GAZ:00619856</oboInOwl:id>
        <rdfs:label>Gernbach</rdfs:label>
    </owl:Class>
    


    <!-- http://purl.obolibrary.org/obo/GAZ_00619857 -->

    <owl:Class rdf:about="http://purl.obolibrary.org/obo/GAZ_00619857">
        <obo:IAO_0000115>A river.</obo:IAO_0000115>
        <oboInOwl:hasOBONamespace>GAZ</oboInOwl:hasOBONamespace>
        <oboInOwl:id>GAZ:00619857</oboInOwl:id>
        <rdfs:label>Gewurzmuhkanal</rdfs:label>
    </owl:Class>
    


    <!-- http://purl.obolibrary.org/obo/GAZ_00619858 -->

    <owl:Class rdf:about="http://purl.obolibrary.org/obo/GAZ_00619858">
        <obo:IAO_0000115>A river.</obo:IAO_0000115>
        <oboInOwl:hasOBONamespace>GAZ</oboInOwl:hasOBONamespace>
        <oboInOwl:id>GAZ:00619858</oboInOwl:id>
        <rdfs:label>Gewurzmuhlbach</rdfs:label>
    </owl:Class>
    


    <!-- http://purl.obolibrary.org/obo/GAZ_00619859 -->

    <owl:Class rdf:about="http://purl.obolibrary.org/obo/GAZ_00619859">
        <obo:IAO_0000115>A river.</obo:IAO_0000115>
        <oboInOwl:hasOBONamespace>GAZ</oboInOwl:hasOBONamespace>
        <oboInOwl:id>GAZ:00619859</oboInOwl:id>
        <rdfs:label>Hacklmuhlbach</rdfs:label>
    </owl:Class>
    


    <!-- http://purl.obolibrary.org/obo/GAZ_00619860 -->

    <owl:Class rdf:about="http://purl.obolibrary.org/obo/GAZ_00619860">
        <obo:IAO_0000115>A river.</obo:IAO_0000115>
        <oboInOwl:hasOBONamespace>GAZ</oboInOwl:hasOBONamespace>
        <oboInOwl:id>GAZ:00619860</oboInOwl:id>
        <rdfs:label>Heiliggeistmuhlbach</rdfs:label>
    </owl:Class>
    


    <!-- http://purl.obolibrary.org/obo/GAZ_00619861 -->

    <owl:Class rdf:about="http://purl.obolibrary.org/obo/GAZ_00619861">
        <obo:IAO_0000115>A river.</obo:IAO_0000115>
        <oboInOwl:hasOBONamespace>GAZ</oboInOwl:hasOBONamespace>
        <oboInOwl:id>GAZ:00619861</oboInOwl:id>
        <rdfs:label>Hochbruckbach</rdfs:label>
    </owl:Class>
    


    <!-- http://purl.obolibrary.org/obo/GAZ_00619862 -->

    <owl:Class rdf:about="http://purl.obolibrary.org/obo/GAZ_00619862">
        <obo:IAO_0000115>A river.</obo:IAO_0000115>
        <oboInOwl:hasOBONamespace>GAZ</oboInOwl:hasOBONamespace>
        <oboInOwl:id>GAZ:00619862</oboInOwl:id>
        <rdfs:label>Hofgrabenbach</rdfs:label>
    </owl:Class>
    


    <!-- http://purl.obolibrary.org/obo/GAZ_00619863 -->

    <owl:Class rdf:about="http://purl.obolibrary.org/obo/GAZ_00619863">
        <obo:IAO_0000115>A river.</obo:IAO_0000115>
        <oboInOwl:hasOBONamespace>GAZ</oboInOwl:hasOBONamespace>
        <oboInOwl:id>GAZ:00619863</oboInOwl:id>
        <rdfs:label>Hofbrunnwerkkanal</rdfs:label>
    </owl:Class>
    


    <!-- http://purl.obolibrary.org/obo/GAZ_00619864 -->

    <owl:Class rdf:about="http://purl.obolibrary.org/obo/GAZ_00619864">
        <obo:IAO_0000115>A river.</obo:IAO_0000115>
        <oboInOwl:hasOBONamespace>GAZ</oboInOwl:hasOBONamespace>
        <oboInOwl:id>GAZ:00619864</oboInOwl:id>
        <rdfs:label>Koglmuhlbach</rdfs:label>
    </owl:Class>
    


    <!-- http://purl.obolibrary.org/obo/GAZ_00619865 -->

    <owl:Class rdf:about="http://purl.obolibrary.org/obo/GAZ_00619865">
        <obo:IAO_0000115>A river.</obo:IAO_0000115>
        <oboInOwl:hasOBONamespace>GAZ</oboInOwl:hasOBONamespace>
        <oboInOwl:id>GAZ:00619865</oboInOwl:id>
        <rdfs:label>Hofhammerschmiedbach</rdfs:label>
    </owl:Class>
    


    <!-- http://purl.obolibrary.org/obo/GAZ_00619866 -->

    <owl:Class rdf:about="http://purl.obolibrary.org/obo/GAZ_00619866">
        <obo:IAO_0000115>A river.</obo:IAO_0000115>
        <oboInOwl:hasOBONamespace>GAZ</oboInOwl:hasOBONamespace>
        <oboInOwl:id>GAZ:00619866</oboInOwl:id>
        <rdfs:label>Hofsagmuhlbach</rdfs:label>
    </owl:Class>
    


    <!-- http://purl.obolibrary.org/obo/GAZ_00619867 -->

    <owl:Class rdf:about="http://purl.obolibrary.org/obo/GAZ_00619867">
        <obo:IAO_0000115>A river.</obo:IAO_0000115>
        <oboInOwl:hasOBONamespace>GAZ</oboInOwl:hasOBONamespace>
        <oboInOwl:id>GAZ:00619867</oboInOwl:id>
        <rdfs:label>Holzgartenkanal</rdfs:label>
    </owl:Class>
    


    <!-- http://purl.obolibrary.org/obo/GAZ_00619868 -->

    <owl:Class rdf:about="http://purl.obolibrary.org/obo/GAZ_00619868">
        <obo:IAO_0000115>A river.</obo:IAO_0000115>
        <oboInOwl:hasOBONamespace>GAZ</oboInOwl:hasOBONamespace>
        <oboInOwl:id>GAZ:00619868</oboInOwl:id>
        <rdfs:label>Hauptmunzkanal</rdfs:label>
    </owl:Class>
    


    <!-- http://purl.obolibrary.org/obo/GAZ_00619869 -->

    <owl:Class rdf:about="http://purl.obolibrary.org/obo/GAZ_00619869">
        <obo:IAO_0000115>A river.</obo:IAO_0000115>
        <oboInOwl:hasOBONamespace>GAZ</oboInOwl:hasOBONamespace>
        <oboInOwl:id>GAZ:00619869</oboInOwl:id>
        <rdfs:label>Hutfabrikkanal</rdfs:label>
    </owl:Class>
    


    <!-- http://purl.obolibrary.org/obo/GAZ_00619870 -->

    <owl:Class rdf:about="http://purl.obolibrary.org/obo/GAZ_00619870">
        <obo:IAO_0000115>A river.</obo:IAO_0000115>
        <oboInOwl:hasOBONamespace>GAZ</oboInOwl:hasOBONamespace>
        <oboInOwl:id>GAZ:00619870</oboInOwl:id>
        <rdfs:label>Kanalbachl</rdfs:label>
    </owl:Class>
    


    <!-- http://purl.obolibrary.org/obo/GAZ_00619871 -->

    <owl:Class rdf:about="http://purl.obolibrary.org/obo/GAZ_00619871">
        <obo:IAO_0000115>A river.</obo:IAO_0000115>
        <oboInOwl:hasOBONamespace>GAZ</oboInOwl:hasOBONamespace>
        <oboInOwl:id>GAZ:00619871</oboInOwl:id>
        <rdfs:label>Kaiblmuhlbach</rdfs:label>
    </owl:Class>
    


    <!-- http://purl.obolibrary.org/obo/GAZ_00619872 -->

    <owl:Class rdf:about="http://purl.obolibrary.org/obo/GAZ_00619872">
        <obo:IAO_0000115>A river.</obo:IAO_0000115>
        <oboInOwl:hasOBONamespace>GAZ</oboInOwl:hasOBONamespace>
        <oboInOwl:id>GAZ:00619872</oboInOwl:id>
        <rdfs:label>Kainzmuhlbach</rdfs:label>
    </owl:Class>
    


    <!-- http://purl.obolibrary.org/obo/GAZ_00619873 -->

    <owl:Class rdf:about="http://purl.obolibrary.org/obo/GAZ_00619873">
        <obo:IAO_0000115>A river.</obo:IAO_0000115>
        <oboInOwl:hasOBONamespace>GAZ</oboInOwl:hasOBONamespace>
        <oboInOwl:id>GAZ:00619873</oboInOwl:id>
        <rdfs:label>Kalblmuhlbach</rdfs:label>
    </owl:Class>
    


    <!-- http://purl.obolibrary.org/obo/GAZ_00619874 -->

    <owl:Class rdf:about="http://purl.obolibrary.org/obo/GAZ_00619874">
        <obo:IAO_0000115>A river.</obo:IAO_0000115>
        <oboInOwl:hasOBONamespace>GAZ</oboInOwl:hasOBONamespace>
        <oboInOwl:id>GAZ:00619874</oboInOwl:id>
        <rdfs:label>Kaltenbach</rdfs:label>
    </owl:Class>
    


    <!-- http://purl.obolibrary.org/obo/GAZ_00619875 -->

    <owl:Class rdf:about="http://purl.obolibrary.org/obo/GAZ_00619875">
        <obo:IAO_0000115>A river.</obo:IAO_0000115>
        <oboInOwl:hasOBONamespace>GAZ</oboInOwl:hasOBONamespace>
        <oboInOwl:id>GAZ:00619875</oboInOwl:id>
        <rdfs:label>Turkengraben</rdfs:label>
    </owl:Class>
    


    <!-- http://purl.obolibrary.org/obo/GAZ_00619877 -->

    <owl:Class rdf:about="http://purl.obolibrary.org/obo/GAZ_00619877">
        <obo:IAO_0000115>A river.</obo:IAO_0000115>
        <oboInOwl:hasOBONamespace>GAZ</oboInOwl:hasOBONamespace>
        <oboInOwl:id>GAZ:00619877</oboInOwl:id>
        <rdfs:label>Katzenbach</rdfs:label>
    </owl:Class>
    


    <!-- http://purl.obolibrary.org/obo/GAZ_00619878 -->

    <owl:Class rdf:about="http://purl.obolibrary.org/obo/GAZ_00619878">
        <obo:IAO_0000115>A river.</obo:IAO_0000115>
        <oboInOwl:hasOBONamespace>GAZ</oboInOwl:hasOBONamespace>
        <oboInOwl:id>GAZ:00619878</oboInOwl:id>
        <rdfs:label>Krankenhausbachl</rdfs:label>
    </owl:Class>
    


    <!-- http://purl.obolibrary.org/obo/GAZ_00619879 -->

    <owl:Class rdf:about="http://purl.obolibrary.org/obo/GAZ_00619879">
        <obo:IAO_0000115>A river.</obo:IAO_0000115>
        <oboInOwl:hasOBONamespace>GAZ</oboInOwl:hasOBONamespace>
        <oboInOwl:id>GAZ:00619879</oboInOwl:id>
        <rdfs:label>Laimbach</rdfs:label>
    </owl:Class>
    


    <!-- http://purl.obolibrary.org/obo/GAZ_00619880 -->

    <owl:Class rdf:about="http://purl.obolibrary.org/obo/GAZ_00619880">
        <obo:IAO_0000115>A river.</obo:IAO_0000115>
        <oboInOwl:hasOBONamespace>GAZ</oboInOwl:hasOBONamespace>
        <oboInOwl:id>GAZ:00619880</oboInOwl:id>
        <rdfs:label>Lazarettbach</rdfs:label>
    </owl:Class>
    


    <!-- http://purl.obolibrary.org/obo/GAZ_00619881 -->

    <owl:Class rdf:about="http://purl.obolibrary.org/obo/GAZ_00619881">
        <obo:IAO_0000115>A river.</obo:IAO_0000115>
        <oboInOwl:hasOBONamespace>GAZ</oboInOwl:hasOBONamespace>
        <oboInOwl:id>GAZ:00619881</oboInOwl:id>
        <rdfs:label>Malzmuhlbach</rdfs:label>
    </owl:Class>
    


    <!-- http://purl.obolibrary.org/obo/GAZ_00619882 -->

    <owl:Class rdf:about="http://purl.obolibrary.org/obo/GAZ_00619882">
        <obo:IAO_0000115>A river.</obo:IAO_0000115>
        <oboInOwl:hasOBONamespace>GAZ</oboInOwl:hasOBONamespace>
        <oboInOwl:id>GAZ:00619882</oboInOwl:id>
        <rdfs:label>Munzbachl</rdfs:label>
    </owl:Class>
    


    <!-- http://purl.obolibrary.org/obo/GAZ_00619883 -->

    <owl:Class rdf:about="http://purl.obolibrary.org/obo/GAZ_00619883">
        <obo:IAO_0000115>A river.</obo:IAO_0000115>
        <oboInOwl:hasOBONamespace>GAZ</oboInOwl:hasOBONamespace>
        <oboInOwl:id>GAZ:00619883</oboInOwl:id>
        <rdfs:label>Muffatbrunnhauskanal</rdfs:label>
    </owl:Class>
    


    <!-- http://purl.obolibrary.org/obo/GAZ_00619885 -->

    <owl:Class rdf:about="http://purl.obolibrary.org/obo/GAZ_00619885">
        <obo:IAO_0000115>A river.</obo:IAO_0000115>
        <oboInOwl:hasOBONamespace>GAZ</oboInOwl:hasOBONamespace>
        <oboInOwl:id>GAZ:00619885</oboInOwl:id>
        <rdfs:label>Papiererbach</rdfs:label>
    </owl:Class>
    


    <!-- http://purl.obolibrary.org/obo/GAZ_00619886 -->

    <owl:Class rdf:about="http://purl.obolibrary.org/obo/GAZ_00619886">
        <obo:IAO_0000115>A river.</obo:IAO_0000115>
        <oboInOwl:hasOBONamespace>GAZ</oboInOwl:hasOBONamespace>
        <oboInOwl:id>GAZ:00619886</oboInOwl:id>
        <rdfs:label>Palaisbachl</rdfs:label>
    </owl:Class>
    


    <!-- http://purl.obolibrary.org/obo/GAZ_00619887 -->

    <owl:Class rdf:about="http://purl.obolibrary.org/obo/GAZ_00619887">
        <obo:IAO_0000115>A river.</obo:IAO_0000115>
        <oboInOwl:hasOBONamespace>GAZ</oboInOwl:hasOBONamespace>
        <oboInOwl:id>GAZ:00619887</oboInOwl:id>
        <rdfs:label>Pfisterbach</rdfs:label>
    </owl:Class>
    


    <!-- http://purl.obolibrary.org/obo/GAZ_00619888 -->

    <owl:Class rdf:about="http://purl.obolibrary.org/obo/GAZ_00619888">
        <obo:IAO_0000115>A river.</obo:IAO_0000115>
        <oboInOwl:hasOBONamespace>GAZ</oboInOwl:hasOBONamespace>
        <oboInOwl:id>GAZ:00619888</oboInOwl:id>
        <rdfs:label>Rossschwemmbach</rdfs:label>
    </owl:Class>
    


    <!-- http://purl.obolibrary.org/obo/GAZ_00619889 -->

    <owl:Class rdf:about="http://purl.obolibrary.org/obo/GAZ_00619889">
        <obo:IAO_0000115>A river.</obo:IAO_0000115>
        <oboInOwl:hasOBONamespace>GAZ</oboInOwl:hasOBONamespace>
        <oboInOwl:id>GAZ:00619889</oboInOwl:id>
        <rdfs:label>Stadthammerschmiedbach</rdfs:label>
    </owl:Class>
    


    <!-- http://purl.obolibrary.org/obo/GAZ_00619890 -->

    <owl:Class rdf:about="http://purl.obolibrary.org/obo/GAZ_00619890">
        <obo:IAO_0000115>A river.</obo:IAO_0000115>
        <oboInOwl:hasOBONamespace>GAZ</oboInOwl:hasOBONamespace>
        <oboInOwl:id>GAZ:00619890</oboInOwl:id>
        <rdfs:label>Steinsagkanal</rdfs:label>
    </owl:Class>
    


    <!-- http://purl.obolibrary.org/obo/GAZ_00619891 -->

    <owl:Class rdf:about="http://purl.obolibrary.org/obo/GAZ_00619891">
        <obo:IAO_0000115>A river.</obo:IAO_0000115>
        <oboInOwl:hasOBONamespace>GAZ</oboInOwl:hasOBONamespace>
        <oboInOwl:id>GAZ:00619891</oboInOwl:id>
        <rdfs:label>Strihhannerbach</rdfs:label>
    </owl:Class>
    


    <!-- http://purl.obolibrary.org/obo/GAZ_00619892 -->

    <owl:Class rdf:about="http://purl.obolibrary.org/obo/GAZ_00619892">
        <obo:IAO_0000115>A river.</obo:IAO_0000115>
        <oboInOwl:hasOBONamespace>GAZ</oboInOwl:hasOBONamespace>
        <oboInOwl:id>GAZ:00619892</oboInOwl:id>
        <rdfs:label>Stadtmuhlbach</rdfs:label>
    </owl:Class>
    


    <!-- http://purl.obolibrary.org/obo/GAZ_00619893 -->

    <owl:Class rdf:about="http://purl.obolibrary.org/obo/GAZ_00619893">
        <obo:IAO_0000115>A river.</obo:IAO_0000115>
        <oboInOwl:hasOBONamespace>GAZ</oboInOwl:hasOBONamespace>
        <oboInOwl:id>GAZ:00619893</oboInOwl:id>
        <rdfs:label>Stadtsagmuhlbach</rdfs:label>
    </owl:Class>
    


    <!-- http://purl.obolibrary.org/obo/GAZ_00619894 -->

    <owl:Class rdf:about="http://purl.obolibrary.org/obo/GAZ_00619894">
        <obo:IAO_0000115>A river.</obo:IAO_0000115>
        <oboInOwl:hasOBONamespace>GAZ</oboInOwl:hasOBONamespace>
        <oboInOwl:id>GAZ:00619894</oboInOwl:id>
        <rdfs:label>Triftkanal</rdfs:label>
    </owl:Class>
    


    <!-- http://purl.obolibrary.org/obo/GAZ_00619895 -->

    <owl:Class rdf:about="http://purl.obolibrary.org/obo/GAZ_00619895">
        <obo:IAO_0000115>A river.</obo:IAO_0000115>
        <oboInOwl:hasOBONamespace>GAZ</oboInOwl:hasOBONamespace>
        <oboInOwl:id>GAZ:00619895</oboInOwl:id>
        <rdfs:label>Triftkanal-Auslaufer</rdfs:label>
    </owl:Class>
    


    <!-- http://purl.obolibrary.org/obo/GAZ_00619896 -->

    <owl:Class rdf:about="http://purl.obolibrary.org/obo/GAZ_00619896">
        <obo:IAO_0000115>A river.</obo:IAO_0000115>
        <oboInOwl:hasOBONamespace>GAZ</oboInOwl:hasOBONamespace>
        <oboInOwl:id>GAZ:00619896</oboInOwl:id>
        <rdfs:label>Wuhrbach</rdfs:label>
    </owl:Class>
    


    <!-- 
    ///////////////////////////////////////////////////////////////////////////////////////
    //
    // Individuals
    //
    ///////////////////////////////////////////////////////////////////////////////////////
     -->

    


    <!-- http://purl.obolibrary.org/obo/GAZ_00002952 -->

    <owl:NamedIndividual rdf:about="http://purl.obolibrary.org/obo/GAZ_00002952">
        <obo:IAO_0000115>A landlocked country in the Carpathian Basin of Central Europe, bordered by Austria, Slovakia, Ukraine, Romania, Serbia, Croatia, and Slovenia. Its capital is Budapest. Hungary is divided into 19 counties (megyek, singular: megye). In addition, the capital city (fovaros), Budapest, is independent of any county government. The counties are further subdivided into 173 subregions (kistersegek), and Budapest is comprised of its own subregion. Since 1996, the counties and City of Budapest have been grouped into 7 regions for statistical and development purposes. These seven regions constitute NUTS second-level units of Hungary.</obo:IAO_0000115>
        <oboInOwl:hasOBONamespace>GAZ</oboInOwl:hasOBONamespace>
        <oboInOwl:id>GAZ:00002952</oboInOwl:id>
        <rdfs:label>Hungary</rdfs:label>
    </owl:NamedIndividual>
    


    <!-- http://purl.obolibrary.org/obo/GAZ_00003594 -->

    <owl:NamedIndividual rdf:about="http://purl.obolibrary.org/obo/GAZ_00003594">
        <obo:RO_0001025 rdf:resource="http://purl.obolibrary.org/obo/GAZ_00002952"/>
    </owl:NamedIndividual>
    


    <!-- http://purl.obolibrary.org/obo/GAZ_00003595 -->

    <owl:NamedIndividual rdf:about="http://purl.obolibrary.org/obo/GAZ_00003595"/>
    


    <!-- http://purl.obolibrary.org/obo/GAZ_00003596 -->

    <owl:NamedIndividual rdf:about="http://purl.obolibrary.org/obo/GAZ_00003596"/>
    


    <!-- http://purl.obolibrary.org/obo/GAZ_00003597 -->

    <owl:NamedIndividual rdf:about="http://purl.obolibrary.org/obo/GAZ_00003597"/>
    


    <!-- http://purl.obolibrary.org/obo/GAZ_00003598 -->

    <owl:NamedIndividual rdf:about="http://purl.obolibrary.org/obo/GAZ_00003598"/>
    


    <!-- http://purl.obolibrary.org/obo/GAZ_00003599 -->

    <owl:NamedIndividual rdf:about="http://purl.obolibrary.org/obo/GAZ_00003599"/>
    


    <!-- http://purl.obolibrary.org/obo/GAZ_00003600 -->

    <owl:NamedIndividual rdf:about="http://purl.obolibrary.org/obo/GAZ_00003600"/>
    


    <!-- http://purl.obolibrary.org/obo/GAZ_00003601 -->

    <owl:NamedIndividual rdf:about="http://purl.obolibrary.org/obo/GAZ_00003601"/>
    


    <!-- http://purl.obolibrary.org/obo/GAZ_00003602 -->

    <owl:NamedIndividual rdf:about="http://purl.obolibrary.org/obo/GAZ_00003602">
        <rdf:type rdf:resource="http://purl.obolibrary.org/obo/ENVO_00000856"/>
        <obo:RO_0001025 rdf:resource="http://purl.obolibrary.org/obo/GAZ_00007375"/>
    </owl:NamedIndividual>
    


    <!-- http://purl.obolibrary.org/obo/GAZ_00003603 -->

    <owl:NamedIndividual rdf:about="http://purl.obolibrary.org/obo/GAZ_00003603">
        <obo:RO_0001025 rdf:resource="http://purl.obolibrary.org/obo/GAZ_00002952"/>
    </owl:NamedIndividual>
    


    <!-- http://purl.obolibrary.org/obo/GAZ_00004702 -->

    <owl:NamedIndividual rdf:about="http://purl.obolibrary.org/obo/GAZ_00004702">
        <obo:RO_0001025 rdf:resource="http://purl.obolibrary.org/obo/GAZ_00007378"/>
    </owl:NamedIndividual>
    


    <!-- http://purl.obolibrary.org/obo/GAZ_00004703 -->

    <owl:NamedIndividual rdf:about="http://purl.obolibrary.org/obo/GAZ_00004703">
        <obo:RO_0001025 rdf:resource="http://purl.obolibrary.org/obo/GAZ_00002952"/>
        <oboInOwl:hasOBONamespace>GAZ</oboInOwl:hasOBONamespace>
        <oboInOwl:id>GAZ:00004703</oboInOwl:id>
        <rdfs:label>Kolso-to</rdfs:label>
    </owl:NamedIndividual>
    


    <!-- http://purl.obolibrary.org/obo/GAZ_00005067 -->

    <owl:NamedIndividual rdf:about="http://purl.obolibrary.org/obo/GAZ_00005067">
        <obo:RO_0001025 rdf:resource="http://purl.obolibrary.org/obo/GAZ_00061809"/>
        <obo:IAO_0000115>A mountain range which forms a natural border between Slovakia and Poland. They occupy an area of 750 km2, the major part (600 km2) of which lies in Slovakia. The highest mountain is Gerlachovsky stit at 2,655m, located in Slovakia. The north-western peak of Rysy (2,499m) is the highest Polish mountain.</obo:IAO_0000115>
        <oboInOwl:hasOBONamespace>GAZ</oboInOwl:hasOBONamespace>
        <oboInOwl:id>GAZ:00005067</oboInOwl:id>
        <rdfs:label>Tatras Mountains</rdfs:label>
    </owl:NamedIndividual>
    


    <!-- http://purl.obolibrary.org/obo/GAZ_00005403 -->

    <owl:NamedIndividual rdf:about="http://purl.obolibrary.org/obo/GAZ_00005403">
        <obo:RO_0001025 rdf:resource="http://purl.obolibrary.org/obo/GAZ_00061809"/>
        <obo:IAO_0000115>A low, about 100 km long, mountain range, part of the Carpathian Mountains. The mountains are situated in Western Slovakia, covering the area from Bratislava to Nove Mesto nad Vahom, and a very small part called Hundsheimer Berge (or Hainburger Berge) is situated in northeastern Austria. They are bordered by Zahorie Lowland in the west and Danubian Lowland in the east.</obo:IAO_0000115>
        <oboInOwl:hasOBONamespace>GAZ</oboInOwl:hasOBONamespace>
        <oboInOwl:id>GAZ:00005403</oboInOwl:id>
        <rdfs:label>Little Carpathians</rdfs:label>
    </owl:NamedIndividual>
    


    <!-- http://purl.obolibrary.org/obo/GAZ_00007375 -->

    <owl:NamedIndividual rdf:about="http://purl.obolibrary.org/obo/GAZ_00007375">
        <obo:RO_0001025 rdf:resource="http://purl.obolibrary.org/obo/GAZ_00007377"/>
        <obo:IAO_0000115>A peninsula into Lake Balaton on its N shore.</obo:IAO_0000115>
        <oboInOwl:hasOBONamespace>GAZ</oboInOwl:hasOBONamespace>
        <oboInOwl:id>GAZ:00007375</oboInOwl:id>
        <rdfs:label>Tihany Peninsula</rdfs:label>
    </owl:NamedIndividual>
    


    <!-- http://purl.obolibrary.org/obo/GAZ_00007377 -->

    <owl:NamedIndividual rdf:about="http://purl.obolibrary.org/obo/GAZ_00007377">
        <obo:RO_0001025 rdf:resource="http://purl.obolibrary.org/obo/GAZ_00003596"/>
        <oboInOwl:hasOBONamespace>GAZ</oboInOwl:hasOBONamespace>
        <oboInOwl:id>GAZ:00007377</oboInOwl:id>
        <rdfs:label>Veszprem County</rdfs:label>
    </owl:NamedIndividual>
    


    <!-- http://purl.obolibrary.org/obo/GAZ_00007378 -->

    <owl:NamedIndividual rdf:about="http://purl.obolibrary.org/obo/GAZ_00007378">
        <obo:RO_0001025 rdf:resource="http://purl.obolibrary.org/obo/GAZ_00003596"/>
        <oboInOwl:hasOBONamespace>GAZ</oboInOwl:hasOBONamespace>
        <oboInOwl:id>GAZ:00007378</oboInOwl:id>
        <rdfs:label>Komarom-Esztergom County</rdfs:label>
    </owl:NamedIndividual>
    


    <!-- http://purl.obolibrary.org/obo/GAZ_00007778 -->

    <owl:NamedIndividual rdf:about="http://purl.obolibrary.org/obo/GAZ_00007778">
        <obo:RO_0001025 rdf:resource="http://purl.obolibrary.org/obo/GAZ_00002952"/>
        <obo:IAO_0000115>A lake, located in Hungary. The Zala River provides the largest inflow of water to the lake, and the canalized Sio is the only outflow.</obo:IAO_0000115>
        <oboInOwl:hasOBONamespace>GAZ</oboInOwl:hasOBONamespace>
        <oboInOwl:id>GAZ:00007778</oboInOwl:id>
        <rdfs:label>Lake Balaton</rdfs:label>
    </owl:NamedIndividual>
    


    <!-- http://purl.obolibrary.org/obo/GAZ_00007973 -->

    <owl:NamedIndividual rdf:about="http://purl.obolibrary.org/obo/GAZ_00007973">
        <obo:RO_0001025 rdf:resource="http://purl.obolibrary.org/obo/GAZ_00056819"/>
        <obo:IAO_0000115>A mountain range in central Slovakia. It is located south of the High Tatras, from which it is separated by the valley of the Vah River. The valley formed by the Hron River is situated south of the Low Tatras range. The ridge runs west-eastwards and is about 80 km long.</obo:IAO_0000115>
        <oboInOwl:hasOBONamespace>GAZ</oboInOwl:hasOBONamespace>
        <oboInOwl:id>GAZ:00007973</oboInOwl:id>
        <rdfs:label>Low Tatras</rdfs:label>
    </owl:NamedIndividual>
    


    <!-- http://purl.obolibrary.org/obo/GAZ_00007974 -->

    <owl:NamedIndividual rdf:about="http://purl.obolibrary.org/obo/GAZ_00007974">
        <obo:RO_0001025 rdf:resource="http://purl.obolibrary.org/obo/GAZ_00056819"/>
        <obo:IAO_0000115>A mountain range on the borders between Slovakia and Poland. They are a part of the Eastern Tatras Mountains.</obo:IAO_0000115>
        <oboInOwl:hasOBONamespace>GAZ</oboInOwl:hasOBONamespace>
        <oboInOwl:id>GAZ:00007974</oboInOwl:id>
        <rdfs:label>High Tatras</rdfs:label>
    </owl:NamedIndividual>
    


    <!-- http://purl.obolibrary.org/obo/GAZ_00007975 -->

    <owl:NamedIndividual rdf:about="http://purl.obolibrary.org/obo/GAZ_00007975">
        <obo:RO_0001025 rdf:resource="http://purl.obolibrary.org/obo/GAZ_00007976"/>
        <obo:IAO_0000115>An ice cave in the Demanovska Valley (Low Tatra) in Slovakia.</obo:IAO_0000115>
        <oboInOwl:hasOBONamespace>GAZ</oboInOwl:hasOBONamespace>
        <oboInOwl:id>GAZ:00007975</oboInOwl:id>
        <rdfs:label>Demanovska Ice Cave</rdfs:label>
    </owl:NamedIndividual>
    


    <!-- http://purl.obolibrary.org/obo/GAZ_00007976 -->

    <owl:NamedIndividual rdf:about="http://purl.obolibrary.org/obo/GAZ_00007976">
        <obo:RO_0001025 rdf:resource="http://purl.obolibrary.org/obo/GAZ_00007973"/>
        <oboInOwl:hasOBONamespace>GAZ</oboInOwl:hasOBONamespace>
        <oboInOwl:id>GAZ:00007976</oboInOwl:id>
        <rdfs:label>Demanovska Valley</rdfs:label>
    </owl:NamedIndividual>
    


    <!-- http://purl.obolibrary.org/obo/GAZ_00008479 -->

    <owl:NamedIndividual rdf:about="http://purl.obolibrary.org/obo/GAZ_00008479">
        <obo:RO_0001025 rdf:resource="http://purl.obolibrary.org/obo/GAZ_00007377"/>
    </owl:NamedIndividual>
    


    <!-- http://purl.obolibrary.org/obo/GAZ_00008480 -->

    <owl:NamedIndividual rdf:about="http://purl.obolibrary.org/obo/GAZ_00008480">
        <obo:RO_0001025 rdf:resource="http://purl.obolibrary.org/obo/GAZ_00002952"/>
        <oboInOwl:hasOBONamespace>GAZ</oboInOwl:hasOBONamespace>
        <oboInOwl:id>GAZ:00008480</oboInOwl:id>
        <rdfs:label>Szent Gyorgy-hedy</rdfs:label>
    </owl:NamedIndividual>
    


    <!-- http://purl.obolibrary.org/obo/GAZ_00010079 -->

    <owl:NamedIndividual rdf:about="http://purl.obolibrary.org/obo/GAZ_00010079">
        <obo:RO_0001025 rdf:resource="http://purl.obolibrary.org/obo/GAZ_00003599"/>
        <oboInOwl:hasOBONamespace>GAZ</oboInOwl:hasOBONamespace>
        <oboInOwl:id>GAZ:00010079</oboInOwl:id>
        <rdfs:label>Csongrad County</rdfs:label>
    </owl:NamedIndividual>
    


    <!-- http://purl.obolibrary.org/obo/GAZ_00010080 -->

    <owl:NamedIndividual rdf:about="http://purl.obolibrary.org/obo/GAZ_00010080">
        <obo:RO_0001025 rdf:resource="http://purl.obolibrary.org/obo/GAZ_00010079"/>
    </owl:NamedIndividual>
    


    <!-- http://purl.obolibrary.org/obo/GAZ_00014330 -->

    <owl:NamedIndividual rdf:about="http://purl.obolibrary.org/obo/GAZ_00014330">
        <obo:RO_0001025 rdf:resource="http://purl.obolibrary.org/obo/GAZ_00003599"/>
        <oboInOwl:hasOBONamespace>GAZ</oboInOwl:hasOBONamespace>
        <oboInOwl:id>GAZ:00014330</oboInOwl:id>
        <rdfs:label>Bekes County</rdfs:label>
    </owl:NamedIndividual>
    


    <!-- http://purl.obolibrary.org/obo/GAZ_00014331 -->

    <owl:NamedIndividual rdf:about="http://purl.obolibrary.org/obo/GAZ_00014331">
        <obo:RO_0001025 rdf:resource="http://purl.obolibrary.org/obo/GAZ_00003601"/>
        <oboInOwl:hasOBONamespace>GAZ</oboInOwl:hasOBONamespace>
        <oboInOwl:id>GAZ:00014331</oboInOwl:id>
        <rdfs:label>Borsod-Abauj-Zemplen County</rdfs:label>
    </owl:NamedIndividual>
    


    <!-- http://purl.obolibrary.org/obo/GAZ_00014332 -->

    <owl:NamedIndividual rdf:about="http://purl.obolibrary.org/obo/GAZ_00014332">
        <obo:RO_0001025 rdf:resource="http://purl.obolibrary.org/obo/GAZ_00003600"/>
        <oboInOwl:hasOBONamespace>GAZ</oboInOwl:hasOBONamespace>
        <oboInOwl:id>GAZ:00014332</oboInOwl:id>
        <rdfs:label>Baranya County</rdfs:label>
    </owl:NamedIndividual>
    


    <!-- http://purl.obolibrary.org/obo/GAZ_00014333 -->

    <owl:NamedIndividual rdf:about="http://purl.obolibrary.org/obo/GAZ_00014333">
        <obo:RO_0001025 rdf:resource="http://purl.obolibrary.org/obo/GAZ_00003599"/>
        <oboInOwl:hasOBONamespace>GAZ</oboInOwl:hasOBONamespace>
        <oboInOwl:id>GAZ:00014333</oboInOwl:id>
        <rdfs:label>Bacs-Kiskun County</rdfs:label>
    </owl:NamedIndividual>
    


    <!-- http://purl.obolibrary.org/obo/GAZ_00014334 -->

    <owl:NamedIndividual rdf:about="http://purl.obolibrary.org/obo/GAZ_00014334">
        <obo:RO_0001025 rdf:resource="http://purl.obolibrary.org/obo/GAZ_00003598"/>
        <oboInOwl:hasOBONamespace>GAZ</oboInOwl:hasOBONamespace>
        <oboInOwl:id>GAZ:00014334</oboInOwl:id>
        <rdfs:label>Vas County</rdfs:label>
    </owl:NamedIndividual>
    


    <!-- http://purl.obolibrary.org/obo/GAZ_00014335 -->

    <owl:NamedIndividual rdf:about="http://purl.obolibrary.org/obo/GAZ_00014335">
        <obo:RO_0001025 rdf:resource="http://purl.obolibrary.org/obo/GAZ_00003597"/>
        <oboInOwl:hasOBONamespace>GAZ</oboInOwl:hasOBONamespace>
        <oboInOwl:id>GAZ:00014335</oboInOwl:id>
        <rdfs:label>Hajdu-Bihar County</rdfs:label>
    </owl:NamedIndividual>
    


    <!-- http://purl.obolibrary.org/obo/GAZ_00014336 -->

    <owl:NamedIndividual rdf:about="http://purl.obolibrary.org/obo/GAZ_00014336">
        <obo:RO_0001025 rdf:resource="http://purl.obolibrary.org/obo/GAZ_00003601"/>
        <oboInOwl:hasOBONamespace>GAZ</oboInOwl:hasOBONamespace>
        <oboInOwl:id>GAZ:00014336</oboInOwl:id>
        <rdfs:label>Nograd County</rdfs:label>
    </owl:NamedIndividual>
    


    <!-- http://purl.obolibrary.org/obo/GAZ_00014337 -->

    <owl:NamedIndividual rdf:about="http://purl.obolibrary.org/obo/GAZ_00014337">
        <obo:RO_0001025 rdf:resource="http://purl.obolibrary.org/obo/GAZ_00003597"/>
        <oboInOwl:hasOBONamespace>GAZ</oboInOwl:hasOBONamespace>
        <oboInOwl:id>GAZ:00014337</oboInOwl:id>
        <rdfs:label>Jasz-Nagykun-Szolnok County</rdfs:label>
    </owl:NamedIndividual>
    


    <!-- http://purl.obolibrary.org/obo/GAZ_00014338 -->

    <owl:NamedIndividual rdf:about="http://purl.obolibrary.org/obo/GAZ_00014338">
        <obo:RO_0001025 rdf:resource="http://purl.obolibrary.org/obo/GAZ_00003597"/>
        <oboInOwl:hasOBONamespace>GAZ</oboInOwl:hasOBONamespace>
        <oboInOwl:id>GAZ:00014338</oboInOwl:id>
        <rdfs:label>Szabolcs-Szatmar-Bereg County</rdfs:label>
    </owl:NamedIndividual>
    


    <!-- http://purl.obolibrary.org/obo/GAZ_00014339 -->

    <owl:NamedIndividual rdf:about="http://purl.obolibrary.org/obo/GAZ_00014339">
        <obo:RO_0001025 rdf:resource="http://purl.obolibrary.org/obo/GAZ_00003601"/>
        <oboInOwl:hasOBONamespace>GAZ</oboInOwl:hasOBONamespace>
        <oboInOwl:id>GAZ:00014339</oboInOwl:id>
        <rdfs:label>Heves County</rdfs:label>
    </owl:NamedIndividual>
    


    <!-- http://purl.obolibrary.org/obo/GAZ_00014340 -->

    <owl:NamedIndividual rdf:about="http://purl.obolibrary.org/obo/GAZ_00014340">
        <obo:RO_0001025 rdf:resource="http://purl.obolibrary.org/obo/GAZ_00003598"/>
        <oboInOwl:hasOBONamespace>GAZ</oboInOwl:hasOBONamespace>
        <oboInOwl:id>GAZ:00014340</oboInOwl:id>
        <rdfs:label>Zala County</rdfs:label>
    </owl:NamedIndividual>
    


    <!-- http://purl.obolibrary.org/obo/GAZ_00014341 -->

    <owl:NamedIndividual rdf:about="http://purl.obolibrary.org/obo/GAZ_00014341">
        <obo:RO_0001025 rdf:resource="http://purl.obolibrary.org/obo/GAZ_00003598"/>
        <oboInOwl:hasOBONamespace>GAZ</oboInOwl:hasOBONamespace>
        <oboInOwl:id>GAZ:00014341</oboInOwl:id>
        <rdfs:label>Gyor-Moson-Sopron County</rdfs:label>
    </owl:NamedIndividual>
    


    <!-- http://purl.obolibrary.org/obo/GAZ_00014342 -->

    <owl:NamedIndividual rdf:about="http://purl.obolibrary.org/obo/GAZ_00014342">
        <obo:RO_0001025 rdf:resource="http://purl.obolibrary.org/obo/GAZ_00003595"/>
        <oboInOwl:hasOBONamespace>GAZ</oboInOwl:hasOBONamespace>
        <oboInOwl:id>GAZ:00014342</oboInOwl:id>
        <rdfs:label>Pest County</rdfs:label>
    </owl:NamedIndividual>
    


    <!-- http://purl.obolibrary.org/obo/GAZ_00014343 -->

    <owl:NamedIndividual rdf:about="http://purl.obolibrary.org/obo/GAZ_00014343">
        <obo:RO_0001025 rdf:resource="http://purl.obolibrary.org/obo/GAZ_00003596"/>
        <oboInOwl:hasOBONamespace>GAZ</oboInOwl:hasOBONamespace>
        <oboInOwl:id>GAZ:00014343</oboInOwl:id>
        <rdfs:label>Fejer County</rdfs:label>
    </owl:NamedIndividual>
    


    <!-- http://purl.obolibrary.org/obo/GAZ_00014344 -->

    <owl:NamedIndividual rdf:about="http://purl.obolibrary.org/obo/GAZ_00014344">
        <obo:RO_0001025 rdf:resource="http://purl.obolibrary.org/obo/GAZ_00003600"/>
        <oboInOwl:hasOBONamespace>GAZ</oboInOwl:hasOBONamespace>
        <oboInOwl:id>GAZ:00014344</oboInOwl:id>
        <rdfs:label>Somogy County</rdfs:label>
    </owl:NamedIndividual>
    


    <!-- http://purl.obolibrary.org/obo/GAZ_00014345 -->

    <owl:NamedIndividual rdf:about="http://purl.obolibrary.org/obo/GAZ_00014345">
        <obo:RO_0001025 rdf:resource="http://purl.obolibrary.org/obo/GAZ_00003600"/>
        <oboInOwl:hasOBONamespace>GAZ</oboInOwl:hasOBONamespace>
        <oboInOwl:id>GAZ:00014345</oboInOwl:id>
        <rdfs:label>Tolna County</rdfs:label>
    </owl:NamedIndividual>
    


    <!-- http://purl.obolibrary.org/obo/GAZ_00036861 -->

    <owl:NamedIndividual rdf:about="http://purl.obolibrary.org/obo/GAZ_00036861">
        <obo:RO_0001025 rdf:resource="http://purl.obolibrary.org/obo/GAZ_00003595"/>
    </owl:NamedIndividual>
    


    <!-- http://purl.obolibrary.org/obo/GAZ_00042184 -->

    <owl:NamedIndividual rdf:about="http://purl.obolibrary.org/obo/GAZ_00042184">
        <oboInOwl:hasOBONamespace>GAZ</oboInOwl:hasOBONamespace>
        <oboInOwl:id>GAZ:00042184</oboInOwl:id>
        <rdfs:label>Pozharevski ostrovi</rdfs:label>
    </owl:NamedIndividual>
    


    <!-- http://purl.obolibrary.org/obo/GAZ_00042185 -->

    <owl:NamedIndividual rdf:about="http://purl.obolibrary.org/obo/GAZ_00042185">
        <obo:RO_0001025 rdf:resource="http://purl.obolibrary.org/obo/GAZ_00042191"/>
        <obo:IAO_0000115>An island located in the Danube, off the Bulgarian coast near the town of Belene.</obo:IAO_0000115>
        <oboInOwl:hasOBONamespace>GAZ</oboInOwl:hasOBONamespace>
        <oboInOwl:id>GAZ:00042185</oboInOwl:id>
        <rdfs:label>Belene Island</rdfs:label>
    </owl:NamedIndividual>
    


    <!-- http://purl.obolibrary.org/obo/GAZ_00042186 -->

    <owl:NamedIndividual rdf:about="http://purl.obolibrary.org/obo/GAZ_00042186">
        <obo:RO_0001025 rdf:resource="http://purl.obolibrary.org/obo/GAZ_00042191"/>
        <obo:IAO_0000115>An island located east of the town of Svishtov, opposite the village of Vardim.</obo:IAO_0000115>
        <oboInOwl:hasOBONamespace>GAZ</oboInOwl:hasOBONamespace>
        <oboInOwl:id>GAZ:00042186</oboInOwl:id>
        <rdfs:label>Vardim Island</rdfs:label>
    </owl:NamedIndividual>
    


    <!-- http://purl.obolibrary.org/obo/GAZ_00042187 -->

    <owl:NamedIndividual rdf:about="http://purl.obolibrary.org/obo/GAZ_00042187">
        <obo:IAO_0000115>An island in the River Danube located opposite the Bulgarian town of Kozloduy, it is 7.5 km in length and between 0.5 and 1.6 km in width, with an area of 6.1 km2.</obo:IAO_0000115>
        <oboInOwl:hasOBONamespace>GAZ</oboInOwl:hasOBONamespace>
        <oboInOwl:id>GAZ:00042187</oboInOwl:id>
        <rdfs:label>Kozloduy Island</rdfs:label>
    </owl:NamedIndividual>
    


    <!-- http://purl.obolibrary.org/obo/GAZ_00042188 -->

    <owl:NamedIndividual rdf:about="http://purl.obolibrary.org/obo/GAZ_00042188">
        <oboInOwl:hasOBONamespace>GAZ</oboInOwl:hasOBONamespace>
        <oboInOwl:id>GAZ:00042188</oboInOwl:id>
        <rdfs:label>Mishka Island</rdfs:label>
    </owl:NamedIndividual>
    


    <!-- http://purl.obolibrary.org/obo/GAZ_00042189 -->

    <owl:NamedIndividual rdf:about="http://purl.obolibrary.org/obo/GAZ_00042189">
        <obo:RO_0001025 rdf:resource="http://purl.obolibrary.org/obo/GAZ_00042184"/>
        <oboInOwl:hasOBONamespace>GAZ</oboInOwl:hasOBONamespace>
        <oboInOwl:id>GAZ:00042189</oboInOwl:id>
        <rdfs:label>Golyam Pozharevo Island</rdfs:label>
    </owl:NamedIndividual>
    


    <!-- http://purl.obolibrary.org/obo/GAZ_00042190 -->

    <owl:NamedIndividual rdf:about="http://purl.obolibrary.org/obo/GAZ_00042190">
        <obo:RO_0001025 rdf:resource="http://purl.obolibrary.org/obo/GAZ_00042184"/>
        <oboInOwl:hasOBONamespace>GAZ</oboInOwl:hasOBONamespace>
        <oboInOwl:id>GAZ:00042190</oboInOwl:id>
        <rdfs:label>Malak Pozharevo Island</rdfs:label>
    </owl:NamedIndividual>
    


    <!-- http://purl.obolibrary.org/obo/GAZ_00042191 -->

    <owl:NamedIndividual rdf:about="http://purl.obolibrary.org/obo/GAZ_00042191">
        <oboInOwl:hasOBONamespace>GAZ</oboInOwl:hasOBONamespace>
        <oboInOwl:id>GAZ:00042191</oboInOwl:id>
        <rdfs:label>Belene Archipelago</rdfs:label>
    </owl:NamedIndividual>
    


    <!-- http://purl.obolibrary.org/obo/GAZ_00042216 -->

    <owl:NamedIndividual rdf:about="http://purl.obolibrary.org/obo/GAZ_00042216">
        <obo:IAO_0000115>An island on the Danube river in the Braila County, Romania.</obo:IAO_0000115>
        <oboInOwl:hasOBONamespace>GAZ</oboInOwl:hasOBONamespace>
        <oboInOwl:id>GAZ:00042216</oboInOwl:id>
        <rdfs:label>Insula Mare a Brailei</rdfs:label>
    </owl:NamedIndividual>
    


    <!-- http://purl.obolibrary.org/obo/GAZ_00042217 -->

    <owl:NamedIndividual rdf:about="http://purl.obolibrary.org/obo/GAZ_00042217">
        <obo:IAO_0000115>An island. between the Bratul Borcea and Bratul Ostrov arms of the Danube.</obo:IAO_0000115>
        <oboInOwl:hasOBONamespace>GAZ</oboInOwl:hasOBONamespace>
        <oboInOwl:id>GAZ:00042217</oboInOwl:id>
        <rdfs:label>Balta Ialomitei</rdfs:label>
    </owl:NamedIndividual>
    


    <!-- http://purl.obolibrary.org/obo/GAZ_00042218 -->

    <owl:NamedIndividual rdf:about="http://purl.obolibrary.org/obo/GAZ_00042218">
        <obo:IAO_0000115>The delta of the River Danube. The greater part of the Danube Delta lies in Romania (Tulcea County), while its northern part, on the left bank of the Chilia arm, is situated in Ukraine (Odessa Oblast).</obo:IAO_0000115>
        <oboInOwl:hasOBONamespace>GAZ</oboInOwl:hasOBONamespace>
        <oboInOwl:id>GAZ:00042218</oboInOwl:id>
        <rdfs:label>Danube Delta</rdfs:label>
    </owl:NamedIndividual>
    


    <!-- http://purl.obolibrary.org/obo/GAZ_00042221 -->

    <owl:NamedIndividual rdf:about="http://purl.obolibrary.org/obo/GAZ_00042221">
        <obo:RO_0001025 rdf:resource="http://purl.obolibrary.org/obo/GAZ_00042218"/>
        <obo:IAO_0000115>A group of the lakes on the beach of Black Sea in Romania south of the Danube Delta. It is the largest lake in Romania. It is a complex formed by a few limans and lagoons. The northern subgroup contains freshwater lakes Razelm and Golovita, whereas the southern group is made up of saline lakes.</obo:IAO_0000115>
        <oboInOwl:hasOBONamespace>GAZ</oboInOwl:hasOBONamespace>
        <oboInOwl:id>GAZ:00042221</oboInOwl:id>
        <rdfs:label>Razelm Lakes</rdfs:label>
    </owl:NamedIndividual>
    


    <!-- http://purl.obolibrary.org/obo/GAZ_00042222 -->

    <owl:NamedIndividual rdf:about="http://purl.obolibrary.org/obo/GAZ_00042222">
        <obo:RO_0001025 rdf:resource="http://purl.obolibrary.org/obo/GAZ_00042221"/>
        <obo:IAO_0000115>A freshwater lake.</obo:IAO_0000115>
        <oboInOwl:hasOBONamespace>GAZ</oboInOwl:hasOBONamespace>
        <oboInOwl:id>GAZ:00042222</oboInOwl:id>
        <rdfs:label>Lacul Razelm</rdfs:label>
    </owl:NamedIndividual>
    


    <!-- http://purl.obolibrary.org/obo/GAZ_00042223 -->

    <owl:NamedIndividual rdf:about="http://purl.obolibrary.org/obo/GAZ_00042223">
        <obo:RO_0001025 rdf:resource="http://purl.obolibrary.org/obo/GAZ_00042221"/>
        <obo:IAO_0000115>A freshwater lake.</obo:IAO_0000115>
        <oboInOwl:hasOBONamespace>GAZ</oboInOwl:hasOBONamespace>
        <oboInOwl:id>GAZ:00042223</oboInOwl:id>
        <rdfs:label>Lacul Golovita</rdfs:label>
    </owl:NamedIndividual>
    


    <!-- http://purl.obolibrary.org/obo/GAZ_00042224 -->

    <owl:NamedIndividual rdf:about="http://purl.obolibrary.org/obo/GAZ_00042224">
        <obo:RO_0001025 rdf:resource="http://purl.obolibrary.org/obo/GAZ_00042222"/>
        <obo:IAO_0000115>An island.</obo:IAO_0000115>
        <oboInOwl:hasOBONamespace>GAZ</oboInOwl:hasOBONamespace>
        <oboInOwl:id>GAZ:00042224</oboInOwl:id>
        <rdfs:label>Insula Popina</rdfs:label>
    </owl:NamedIndividual>
    


    <!-- http://purl.obolibrary.org/obo/GAZ_00042225 -->

    <owl:NamedIndividual rdf:about="http://purl.obolibrary.org/obo/GAZ_00042225">
        <obo:RO_0001025 rdf:resource="http://purl.obolibrary.org/obo/GAZ_00042234"/>
        <obo:IAO_0000115>A newly formed island in the Black Sea, right off the coast of the Romanian Danube Delta, off the Sfantu Gheorghe branch. Initially Sacalin was made up of two smaller islands, Sacalinu Mare (Greater Sacalin) and Sacalinu Mic (Lesser Sacalin). In time, however, the two merged into one continuous landmass.</obo:IAO_0000115>
        <oboInOwl:hasOBONamespace>GAZ</oboInOwl:hasOBONamespace>
        <oboInOwl:id>GAZ:00042225</oboInOwl:id>
        <rdfs:label>Sacalin Island</rdfs:label>
    </owl:NamedIndividual>
    


    <!-- http://purl.obolibrary.org/obo/GAZ_00042226 -->

    <owl:NamedIndividual rdf:about="http://purl.obolibrary.org/obo/GAZ_00042226">
        <obo:RO_0001025 rdf:resource="http://purl.obolibrary.org/obo/GAZ_00042225"/>
        <oboInOwl:hasOBONamespace>GAZ</oboInOwl:hasOBONamespace>
        <oboInOwl:id>GAZ:00042226</oboInOwl:id>
        <rdfs:label>Sacalinu Mare</rdfs:label>
    </owl:NamedIndividual>
    


    <!-- http://purl.obolibrary.org/obo/GAZ_00042227 -->

    <owl:NamedIndividual rdf:about="http://purl.obolibrary.org/obo/GAZ_00042227">
        <obo:RO_0001025 rdf:resource="http://purl.obolibrary.org/obo/GAZ_00042225"/>
        <oboInOwl:hasOBONamespace>GAZ</oboInOwl:hasOBONamespace>
        <oboInOwl:id>GAZ:00042227</oboInOwl:id>
        <rdfs:label>Sacalinu Mic</rdfs:label>
    </owl:NamedIndividual>
    


    <!-- http://purl.obolibrary.org/obo/GAZ_00042228 -->

    <owl:NamedIndividual rdf:about="http://purl.obolibrary.org/obo/GAZ_00042228">
        <obo:RO_0001025 rdf:resource="http://purl.obolibrary.org/obo/GAZ_00042218"/>
        <oboInOwl:hasOBONamespace>GAZ</oboInOwl:hasOBONamespace>
        <oboInOwl:id>GAZ:00042228</oboInOwl:id>
        <rdfs:label>Ostrovu Tataru</rdfs:label>
    </owl:NamedIndividual>
    


    <!-- http://purl.obolibrary.org/obo/GAZ_00042231 -->

    <owl:NamedIndividual rdf:about="http://purl.obolibrary.org/obo/GAZ_00042231">
        <obo:RO_0001025 rdf:resource="http://purl.obolibrary.org/obo/GAZ_00042218"/>
        <obo:IAO_0000115>A lagoon in Northern Dobruja, Romania, close to the Black Sea.</obo:IAO_0000115>
        <oboInOwl:hasOBONamespace>GAZ</oboInOwl:hasOBONamespace>
        <oboInOwl:id>GAZ:00042231</oboInOwl:id>
        <rdfs:label>Lacul Sinoe</rdfs:label>
    </owl:NamedIndividual>
    


    <!-- http://purl.obolibrary.org/obo/GAZ_00042232 -->

    <owl:NamedIndividual rdf:about="http://purl.obolibrary.org/obo/GAZ_00042232">
        <obo:RO_0001025 rdf:resource="http://purl.obolibrary.org/obo/GAZ_00042231"/>
        <oboInOwl:hasOBONamespace>GAZ</oboInOwl:hasOBONamespace>
        <oboInOwl:id>GAZ:00042232</oboInOwl:id>
        <rdfs:label>Ceaplace Island</rdfs:label>
    </owl:NamedIndividual>
    


    <!-- http://purl.obolibrary.org/obo/GAZ_00042233 -->

    <owl:NamedIndividual rdf:about="http://purl.obolibrary.org/obo/GAZ_00042233">
        <obo:RO_0001025 rdf:resource="http://purl.obolibrary.org/obo/GAZ_00062827"/>
        <obo:IAO_0000115>The N arm of the Danube in its Delta.</obo:IAO_0000115>
        <oboInOwl:hasOBONamespace>GAZ</oboInOwl:hasOBONamespace>
        <oboInOwl:id>GAZ:00042233</oboInOwl:id>
        <rdfs:label>Chilia Channel</rdfs:label>
    </owl:NamedIndividual>
    


    <!-- http://purl.obolibrary.org/obo/GAZ_00042234 -->

    <owl:NamedIndividual rdf:about="http://purl.obolibrary.org/obo/GAZ_00042234">
        <obo:RO_0001025 rdf:resource="http://purl.obolibrary.org/obo/GAZ_00042218"/>
        <obo:IAO_0000115>The S arm of the Danube in its Delta.</obo:IAO_0000115>
        <oboInOwl:hasOBONamespace>GAZ</oboInOwl:hasOBONamespace>
        <oboInOwl:id>GAZ:00042234</oboInOwl:id>
        <rdfs:label>Sfantu Gheorghe Channel</rdfs:label>
    </owl:NamedIndividual>
    


    <!-- http://purl.obolibrary.org/obo/GAZ_00042235 -->

    <owl:NamedIndividual rdf:about="http://purl.obolibrary.org/obo/GAZ_00042235">
        <obo:RO_0001025 rdf:resource="http://purl.obolibrary.org/obo/GAZ_00062827"/>
        <obo:IAO_0000115>The central arm of the Danube in its Delta.</obo:IAO_0000115>
        <oboInOwl:hasOBONamespace>GAZ</oboInOwl:hasOBONamespace>
        <oboInOwl:id>GAZ:00042235</oboInOwl:id>
        <rdfs:label>Sulina Channel</rdfs:label>
    </owl:NamedIndividual>
    


    <!-- http://purl.obolibrary.org/obo/GAZ_00042236 -->

    <owl:NamedIndividual rdf:about="http://purl.obolibrary.org/obo/GAZ_00042236">
        <oboInOwl:hasOBONamespace>GAZ</oboInOwl:hasOBONamespace>
        <oboInOwl:id>GAZ:00042236</oboInOwl:id>
        <rdfs:label>Moldova Veche Island</rdfs:label>
    </owl:NamedIndividual>
    


    <!-- http://purl.obolibrary.org/obo/GAZ_00042238 -->

    <owl:NamedIndividual rdf:about="http://purl.obolibrary.org/obo/GAZ_00042238">
        <obo:RO_0001025 rdf:resource="http://purl.obolibrary.org/obo/GAZ_00179202"/>
        <obo:IAO_0000115>A group of twelve islands (0.6 ha) which are located in the Gabcikovo Reservoir south of Bratislava, west from the Kalinkovo village. They were built in the years 2006 and 2007 as part of flood-protection of the Slovak capital.</obo:IAO_0000115>
        <oboInOwl:hasOBONamespace>GAZ</oboInOwl:hasOBONamespace>
        <oboInOwl:id>GAZ:00042238</oboInOwl:id>
        <rdfs:label>Benkove ostrovy</rdfs:label>
    </owl:NamedIndividual>
    


    <!-- http://purl.obolibrary.org/obo/GAZ_00043902 -->

    <owl:NamedIndividual rdf:about="http://purl.obolibrary.org/obo/GAZ_00043902">
        <obo:IAO_0000115>An island in the Sava river flowing through central Belgrade the capital city of Serbia. The island belongs to the Belgrade municipality of Cukarica. It is located at the 4th km from the Sava&apos;s confluence into the Danube near the central parts of Belgrade.</obo:IAO_0000115>
        <oboInOwl:hasOBONamespace>GAZ</oboInOwl:hasOBONamespace>
        <oboInOwl:id>GAZ:00043902</oboInOwl:id>
        <rdfs:label>Ada Ciganlija</rdfs:label>
    </owl:NamedIndividual>
    


    <!-- http://purl.obolibrary.org/obo/GAZ_00043905 -->

    <owl:NamedIndividual rdf:about="http://purl.obolibrary.org/obo/GAZ_00043905">
        <obo:IAO_0000115>An ovally shaped river island in the Sava river, a km long and 200 m wide. It is located just north of the central part of the much larger Ada Ciganlija.</obo:IAO_0000115>
        <oboInOwl:hasOBONamespace>GAZ</oboInOwl:hasOBONamespace>
        <oboInOwl:id>GAZ:00043905</oboInOwl:id>
        <rdfs:label>Ada Medica</rdfs:label>
    </owl:NamedIndividual>
    


    <!-- http://purl.obolibrary.org/obo/GAZ_00043907 -->

    <owl:NamedIndividual rdf:about="http://purl.obolibrary.org/obo/GAZ_00043907">
        <obo:IAO_0000115>A projected river island (ada) in Serbia, on the left bank of the Danube. According to the General Urbanistic Plan (GUP) of Belgrade, it will be formed in Belgrade&apos;s municipality of Palilula.</obo:IAO_0000115>
        <oboInOwl:hasOBONamespace>GAZ</oboInOwl:hasOBONamespace>
        <oboInOwl:id>GAZ:00043907</oboInOwl:id>
        <rdfs:label>Caplja Island</rdfs:label>
    </owl:NamedIndividual>
    


    <!-- http://purl.obolibrary.org/obo/GAZ_00043909 -->

    <owl:NamedIndividual rdf:about="http://purl.obolibrary.org/obo/GAZ_00043909">
        <obo:IAO_0000115>A fluvial island (ada) in Serbia, located on the left bank of the Danube. It is part of the Belgrade City proper and belongs to the Belgrade&apos;s municipality of Palilula. The island is floodable, completely covered with forest and without permanent population.</obo:IAO_0000115>
        <oboInOwl:hasOBONamespace>GAZ</oboInOwl:hasOBONamespace>
        <oboInOwl:id>GAZ:00043909</oboInOwl:id>
        <rdfs:label>Kozara Island</rdfs:label>
    </owl:NamedIndividual>
    


    <!-- http://purl.obolibrary.org/obo/GAZ_00043910 -->

    <owl:NamedIndividual rdf:about="http://purl.obolibrary.org/obo/GAZ_00043910">
        <obo:IAO_0000115>The largest Serbian island on the Danube, with an area of 60 km2; 20 km in length and 3 km in width. The island lies east of Belgrade, near Kostolac, and is heavily forested, and uninhabited.</obo:IAO_0000115>
        <oboInOwl:hasOBONamespace>GAZ</oboInOwl:hasOBONamespace>
        <oboInOwl:id>GAZ:00043910</oboInOwl:id>
        <rdfs:label>Ostrvo [Kostolac]</rdfs:label>
    </owl:NamedIndividual>
    


    <!-- http://purl.obolibrary.org/obo/GAZ_00043912 -->

    <owl:NamedIndividual rdf:about="http://purl.obolibrary.org/obo/GAZ_00043912">
        <rdf:type rdf:resource="http://purl.obolibrary.org/obo/ENVO_00000423"/>
        <obo:IAO_0000115>A fluvial island in Serbia, located at the mouth of the Sava river into the Danube. Though uninhabited, it is part of the Belgrade City proper, the capital of Serbia, and belongs to the municipality of Zemun. Great War Island is located at the mouth of the Sava river into the Danube, in the Danube&apos;s widening between the Kalemegdan fortress as the ending section of the Terazije ridge of northernmost part of Sumadija on the west and the low, easternmost sextion of the Syrmia plain, the modern Usce neighborhood of Novi Beograd, on the south.</obo:IAO_0000115>
        <oboInOwl:hasOBONamespace>GAZ</oboInOwl:hasOBONamespace>
        <oboInOwl:id>GAZ:00043912</oboInOwl:id>
        <rdfs:label>Veliko Ratno Ostrvo</rdfs:label>
    </owl:NamedIndividual>
    


    <!-- http://purl.obolibrary.org/obo/GAZ_00043929 -->

    <owl:NamedIndividual rdf:about="http://purl.obolibrary.org/obo/GAZ_00043929">
        <oboInOwl:hasOBONamespace>GAZ</oboInOwl:hasOBONamespace>
        <oboInOwl:id>GAZ:00043929</oboInOwl:id>
        <rdfs:label>Farkas-sziget</rdfs:label>
    </owl:NamedIndividual>
    


    <!-- http://purl.obolibrary.org/obo/GAZ_00043930 -->

    <owl:NamedIndividual rdf:about="http://purl.obolibrary.org/obo/GAZ_00043930">
        <oboInOwl:hasOBONamespace>GAZ</oboInOwl:hasOBONamespace>
        <oboInOwl:id>GAZ:00043930</oboInOwl:id>
        <rdfs:label>Kacsa-sziget</rdfs:label>
    </owl:NamedIndividual>
    


    <!-- http://purl.obolibrary.org/obo/GAZ_00043931 -->

    <owl:NamedIndividual rdf:about="http://purl.obolibrary.org/obo/GAZ_00043931">
        <oboInOwl:hasOBONamespace>GAZ</oboInOwl:hasOBONamespace>
        <oboInOwl:id>GAZ:00043931</oboInOwl:id>
        <rdfs:label>Korom-sziget</rdfs:label>
    </owl:NamedIndividual>
    


    <!-- http://purl.obolibrary.org/obo/GAZ_00043932 -->

    <owl:NamedIndividual rdf:about="http://purl.obolibrary.org/obo/GAZ_00043932">
        <oboInOwl:hasOBONamespace>GAZ</oboInOwl:hasOBONamespace>
        <oboInOwl:id>GAZ:00043932</oboInOwl:id>
        <rdfs:label>Bulati-sziget</rdfs:label>
    </owl:NamedIndividual>
    


    <!-- http://purl.obolibrary.org/obo/GAZ_00043933 -->

    <owl:NamedIndividual rdf:about="http://purl.obolibrary.org/obo/GAZ_00043933">
        <oboInOwl:hasOBONamespace>GAZ</oboInOwl:hasOBONamespace>
        <oboInOwl:id>GAZ:00043933</oboInOwl:id>
        <rdfs:label>Alcsi-sziget</rdfs:label>
    </owl:NamedIndividual>
    


    <!-- http://purl.obolibrary.org/obo/GAZ_00043934 -->

    <owl:NamedIndividual rdf:about="http://purl.obolibrary.org/obo/GAZ_00043934">
        <oboInOwl:hasOBONamespace>GAZ</oboInOwl:hasOBONamespace>
        <oboInOwl:id>GAZ:00043934</oboInOwl:id>
        <rdfs:label>Kis-Tisza-sziget</rdfs:label>
    </owl:NamedIndividual>
    


    <!-- http://purl.obolibrary.org/obo/GAZ_00043935 -->

    <owl:NamedIndividual rdf:about="http://purl.obolibrary.org/obo/GAZ_00043935">
        <oboInOwl:hasOBONamespace>GAZ</oboInOwl:hasOBONamespace>
        <oboInOwl:id>GAZ:00043935</oboInOwl:id>
        <rdfs:label>Arany-sziget</rdfs:label>
    </owl:NamedIndividual>
    


    <!-- http://purl.obolibrary.org/obo/GAZ_00043936 -->

    <owl:NamedIndividual rdf:about="http://purl.obolibrary.org/obo/GAZ_00043936">
        <obo:RO_0001025 rdf:resource="http://purl.obolibrary.org/obo/GAZ_00003594"/>
        <oboInOwl:hasOBONamespace>GAZ</oboInOwl:hasOBONamespace>
        <oboInOwl:id>GAZ:00043936</oboInOwl:id>
        <rdfs:label>Domariba-sziget</rdfs:label>
    </owl:NamedIndividual>
    


    <!-- http://purl.obolibrary.org/obo/GAZ_00043937 -->

    <owl:NamedIndividual rdf:about="http://purl.obolibrary.org/obo/GAZ_00043937">
        <obo:RO_0001025 rdf:resource="http://purl.obolibrary.org/obo/GAZ_00003594"/>
        <oboInOwl:hasOBONamespace>GAZ</oboInOwl:hasOBONamespace>
        <oboInOwl:id>GAZ:00043937</oboInOwl:id>
        <rdfs:label>Pap-sziget</rdfs:label>
    </owl:NamedIndividual>
    


    <!-- http://purl.obolibrary.org/obo/GAZ_00043938 -->

    <owl:NamedIndividual rdf:about="http://purl.obolibrary.org/obo/GAZ_00043938">
        <obo:RO_0001025 rdf:resource="http://purl.obolibrary.org/obo/GAZ_00003594"/>
        <oboInOwl:hasOBONamespace>GAZ</oboInOwl:hasOBONamespace>
        <oboInOwl:id>GAZ:00043938</oboInOwl:id>
        <rdfs:label>Veranka-sziget</rdfs:label>
    </owl:NamedIndividual>
    


    <!-- http://purl.obolibrary.org/obo/GAZ_00043939 -->

    <owl:NamedIndividual rdf:about="http://purl.obolibrary.org/obo/GAZ_00043939">
        <obo:RO_0001025 rdf:resource="http://purl.obolibrary.org/obo/GAZ_00003594"/>
        <oboInOwl:hasOBONamespace>GAZ</oboInOwl:hasOBONamespace>
        <oboInOwl:id>GAZ:00043939</oboInOwl:id>
        <rdfs:label>Szunyog-sziget</rdfs:label>
    </owl:NamedIndividual>
    


    <!-- http://purl.obolibrary.org/obo/GAZ_00043940 -->

    <owl:NamedIndividual rdf:about="http://purl.obolibrary.org/obo/GAZ_00043940">
        <obo:RO_0001025 rdf:resource="http://purl.obolibrary.org/obo/GAZ_00003594"/>
        <oboInOwl:hasOBONamespace>GAZ</oboInOwl:hasOBONamespace>
        <oboInOwl:id>GAZ:00043940</oboInOwl:id>
        <rdfs:label>Cseke-sziget</rdfs:label>
    </owl:NamedIndividual>
    


    <!-- http://purl.obolibrary.org/obo/GAZ_00043941 -->

    <owl:NamedIndividual rdf:about="http://purl.obolibrary.org/obo/GAZ_00043941">
        <obo:RO_0001025 rdf:resource="http://purl.obolibrary.org/obo/GAZ_00003594"/>
        <oboInOwl:hasOBONamespace>GAZ</oboInOwl:hasOBONamespace>
        <oboInOwl:id>GAZ:00043941</oboInOwl:id>
        <rdfs:label>Kohidi-sziget</rdfs:label>
    </owl:NamedIndividual>
    


    <!-- http://purl.obolibrary.org/obo/GAZ_00043942 -->

    <owl:NamedIndividual rdf:about="http://purl.obolibrary.org/obo/GAZ_00043942">
        <obo:RO_0001025 rdf:resource="http://purl.obolibrary.org/obo/GAZ_00003594"/>
        <oboInOwl:hasOBONamespace>GAZ</oboInOwl:hasOBONamespace>
        <oboInOwl:id>GAZ:00043942</oboInOwl:id>
        <rdfs:label>Godi-sziget</rdfs:label>
    </owl:NamedIndividual>
    


    <!-- http://purl.obolibrary.org/obo/GAZ_00043943 -->

    <owl:NamedIndividual rdf:about="http://purl.obolibrary.org/obo/GAZ_00043943">
        <obo:RO_0001025 rdf:resource="http://purl.obolibrary.org/obo/GAZ_00003594"/>
        <oboInOwl:hasOBONamespace>GAZ</oboInOwl:hasOBONamespace>
        <oboInOwl:id>GAZ:00043943</oboInOwl:id>
        <rdfs:label>Felsozatonyi-sziget</rdfs:label>
    </owl:NamedIndividual>
    


    <!-- http://purl.obolibrary.org/obo/GAZ_00043944 -->

    <owl:NamedIndividual rdf:about="http://purl.obolibrary.org/obo/GAZ_00043944">
        <obo:RO_0001025 rdf:resource="http://purl.obolibrary.org/obo/GAZ_00003594"/>
        <oboInOwl:hasOBONamespace>GAZ</oboInOwl:hasOBONamespace>
        <oboInOwl:id>GAZ:00043944</oboInOwl:id>
        <rdfs:label>Lupa-sziget</rdfs:label>
    </owl:NamedIndividual>
    


    <!-- http://purl.obolibrary.org/obo/GAZ_00043945 -->

    <owl:NamedIndividual rdf:about="http://purl.obolibrary.org/obo/GAZ_00043945">
        <obo:RO_0001025 rdf:resource="http://purl.obolibrary.org/obo/GAZ_00003594"/>
        <oboInOwl:hasOBONamespace>GAZ</oboInOwl:hasOBONamespace>
        <oboInOwl:id>GAZ:00043945</oboInOwl:id>
        <rdfs:label>Petofi-sziget</rdfs:label>
    </owl:NamedIndividual>
    


    <!-- http://purl.obolibrary.org/obo/GAZ_00043946 -->

    <owl:NamedIndividual rdf:about="http://purl.obolibrary.org/obo/GAZ_00043946">
        <obo:RO_0001025 rdf:resource="http://purl.obolibrary.org/obo/GAZ_00003594"/>
        <oboInOwl:hasOBONamespace>GAZ</oboInOwl:hasOBONamespace>
        <oboInOwl:id>GAZ:00043946</oboInOwl:id>
        <rdfs:label>Oreg-sziget</rdfs:label>
    </owl:NamedIndividual>
    


    <!-- http://purl.obolibrary.org/obo/GAZ_00043947 -->

    <owl:NamedIndividual rdf:about="http://purl.obolibrary.org/obo/GAZ_00043947">
        <obo:RO_0001025 rdf:resource="http://purl.obolibrary.org/obo/GAZ_00003594"/>
        <oboInOwl:hasOBONamespace>GAZ</oboInOwl:hasOBONamespace>
        <oboInOwl:id>GAZ:00043947</oboInOwl:id>
        <rdfs:label>Martuska-sziget</rdfs:label>
    </owl:NamedIndividual>
    


    <!-- http://purl.obolibrary.org/obo/GAZ_00043948 -->

    <owl:NamedIndividual rdf:about="http://purl.obolibrary.org/obo/GAZ_00043948">
        <obo:RO_0001025 rdf:resource="http://purl.obolibrary.org/obo/GAZ_00003594"/>
        <oboInOwl:hasOBONamespace>GAZ</oboInOwl:hasOBONamespace>
        <oboInOwl:id>GAZ:00043948</oboInOwl:id>
        <rdfs:label>Szalki-sziget</rdfs:label>
    </owl:NamedIndividual>
    


    <!-- http://purl.obolibrary.org/obo/GAZ_00043949 -->

    <owl:NamedIndividual rdf:about="http://purl.obolibrary.org/obo/GAZ_00043949">
        <obo:RO_0001025 rdf:resource="http://purl.obolibrary.org/obo/GAZ_00003594"/>
        <oboInOwl:hasOBONamespace>GAZ</oboInOwl:hasOBONamespace>
        <oboInOwl:id>GAZ:00043949</oboInOwl:id>
        <rdfs:label>Palanki-sziget</rdfs:label>
    </owl:NamedIndividual>
    


    <!-- http://purl.obolibrary.org/obo/GAZ_00043950 -->

    <owl:NamedIndividual rdf:about="http://purl.obolibrary.org/obo/GAZ_00043950">
        <obo:RO_0001025 rdf:resource="http://purl.obolibrary.org/obo/GAZ_00003594"/>
        <oboInOwl:hasOBONamespace>GAZ</oboInOwl:hasOBONamespace>
        <oboInOwl:id>GAZ:00043950</oboInOwl:id>
        <rdfs:label>Nagy-Pandur-sziget</rdfs:label>
    </owl:NamedIndividual>
    


    <!-- http://purl.obolibrary.org/obo/GAZ_00043951 -->

    <owl:NamedIndividual rdf:about="http://purl.obolibrary.org/obo/GAZ_00043951">
        <obo:RO_0001025 rdf:resource="http://purl.obolibrary.org/obo/GAZ_00003594"/>
        <oboInOwl:hasOBONamespace>GAZ</oboInOwl:hasOBONamespace>
        <oboInOwl:id>GAZ:00043951</oboInOwl:id>
        <rdfs:label>Haraszti-sziget</rdfs:label>
    </owl:NamedIndividual>
    


    <!-- http://purl.obolibrary.org/obo/GAZ_00043952 -->

    <owl:NamedIndividual rdf:about="http://purl.obolibrary.org/obo/GAZ_00043952">
        <obo:RO_0001025 rdf:resource="http://purl.obolibrary.org/obo/GAZ_00003594"/>
        <oboInOwl:hasOBONamespace>GAZ</oboInOwl:hasOBONamespace>
        <oboInOwl:id>GAZ:00043952</oboInOwl:id>
        <rdfs:label>Dunasziget</rdfs:label>
    </owl:NamedIndividual>
    


    <!-- http://purl.obolibrary.org/obo/GAZ_00043953 -->

    <owl:NamedIndividual rdf:about="http://purl.obolibrary.org/obo/GAZ_00043953">
        <obo:RO_0001025 rdf:resource="http://purl.obolibrary.org/obo/GAZ_00003594"/>
        <oboInOwl:hasOBONamespace>GAZ</oboInOwl:hasOBONamespace>
        <oboInOwl:id>GAZ:00043953</oboInOwl:id>
        <rdfs:label>Szentendrei-sziget</rdfs:label>
    </owl:NamedIndividual>
    


    <!-- http://purl.obolibrary.org/obo/GAZ_00043954 -->

    <owl:NamedIndividual rdf:about="http://purl.obolibrary.org/obo/GAZ_00043954">
        <obo:RO_0001025 rdf:resource="http://purl.obolibrary.org/obo/GAZ_00003594"/>
        <oboInOwl:hasOBONamespace>GAZ</oboInOwl:hasOBONamespace>
        <oboInOwl:id>GAZ:00043954</oboInOwl:id>
        <rdfs:label>Mohacsi-sziget</rdfs:label>
    </owl:NamedIndividual>
    


    <!-- http://purl.obolibrary.org/obo/GAZ_00043955 -->

    <owl:NamedIndividual rdf:about="http://purl.obolibrary.org/obo/GAZ_00043955">
        <obo:RO_0001025 rdf:resource="http://purl.obolibrary.org/obo/GAZ_00003594"/>
        <oboInOwl:hasOBONamespace>GAZ</oboInOwl:hasOBONamespace>
        <oboInOwl:id>GAZ:00043955</oboInOwl:id>
        <rdfs:label>Taksony-sziget</rdfs:label>
    </owl:NamedIndividual>
    


    <!-- http://purl.obolibrary.org/obo/GAZ_00043956 -->

    <owl:NamedIndividual rdf:about="http://purl.obolibrary.org/obo/GAZ_00043956">
        <obo:RO_0001025 rdf:resource="http://purl.obolibrary.org/obo/GAZ_00003594"/>
        <oboInOwl:hasOBONamespace>GAZ</oboInOwl:hasOBONamespace>
        <oboInOwl:id>GAZ:00043956</oboInOwl:id>
        <rdfs:label>Czuczor-sziget</rdfs:label>
    </owl:NamedIndividual>
    


    <!-- http://purl.obolibrary.org/obo/GAZ_00043957 -->

    <owl:NamedIndividual rdf:about="http://purl.obolibrary.org/obo/GAZ_00043957">
        <obo:RO_0001025 rdf:resource="http://purl.obolibrary.org/obo/GAZ_00003594"/>
        <oboInOwl:hasOBONamespace>GAZ</oboInOwl:hasOBONamespace>
        <oboInOwl:id>GAZ:00043957</oboInOwl:id>
        <rdfs:label>Sport-sziget</rdfs:label>
    </owl:NamedIndividual>
    


    <!-- http://purl.obolibrary.org/obo/GAZ_00043958 -->

    <owl:NamedIndividual rdf:about="http://purl.obolibrary.org/obo/GAZ_00043958">
        <obo:RO_0001025 rdf:resource="http://purl.obolibrary.org/obo/GAZ_00003594"/>
        <obo:RO_0001025 rdf:resource="http://purl.obolibrary.org/obo/GAZ_00036861"/>
        <oboInOwl:hasOBONamespace>GAZ</oboInOwl:hasOBONamespace>
        <oboInOwl:id>GAZ:00043958</oboInOwl:id>
        <rdfs:label>Margitsziget</rdfs:label>
    </owl:NamedIndividual>
    


    <!-- http://purl.obolibrary.org/obo/GAZ_00043959 -->

    <owl:NamedIndividual rdf:about="http://purl.obolibrary.org/obo/GAZ_00043959">
        <obo:RO_0001025 rdf:resource="http://purl.obolibrary.org/obo/GAZ_00003594"/>
        <obo:RO_0001025 rdf:resource="http://purl.obolibrary.org/obo/GAZ_00036861"/>
        <oboInOwl:hasOBONamespace>GAZ</oboInOwl:hasOBONamespace>
        <oboInOwl:id>GAZ:00043959</oboInOwl:id>
        <rdfs:label>Obudai-sziget</rdfs:label>
    </owl:NamedIndividual>
    


    <!-- http://purl.obolibrary.org/obo/GAZ_00043960 -->

    <owl:NamedIndividual rdf:about="http://purl.obolibrary.org/obo/GAZ_00043960">
        <obo:RO_0001025 rdf:resource="http://purl.obolibrary.org/obo/GAZ_00003594"/>
        <obo:RO_0001025 rdf:resource="http://purl.obolibrary.org/obo/GAZ_00036861"/>
        <oboInOwl:hasOBONamespace>GAZ</oboInOwl:hasOBONamespace>
        <oboInOwl:id>GAZ:00043960</oboInOwl:id>
        <rdfs:label>Molnar-sziget</rdfs:label>
    </owl:NamedIndividual>
    


    <!-- http://purl.obolibrary.org/obo/GAZ_00043961 -->

    <owl:NamedIndividual rdf:about="http://purl.obolibrary.org/obo/GAZ_00043961">
        <obo:RO_0001025 rdf:resource="http://purl.obolibrary.org/obo/GAZ_00003594"/>
        <obo:RO_0001025 rdf:resource="http://purl.obolibrary.org/obo/GAZ_00036861"/>
        <oboInOwl:hasOBONamespace>GAZ</oboInOwl:hasOBONamespace>
        <oboInOwl:id>GAZ:00043961</oboInOwl:id>
        <rdfs:label>Csepel-sziget</rdfs:label>
    </owl:NamedIndividual>
    


    <!-- http://purl.obolibrary.org/obo/GAZ_00043962 -->

    <owl:NamedIndividual rdf:about="http://purl.obolibrary.org/obo/GAZ_00043962">
        <obo:RO_0001025 rdf:resource="http://purl.obolibrary.org/obo/GAZ_00003594"/>
        <obo:RO_0001025 rdf:resource="http://purl.obolibrary.org/obo/GAZ_00036861"/>
        <oboInOwl:hasOBONamespace>GAZ</oboInOwl:hasOBONamespace>
        <oboInOwl:id>GAZ:00043962</oboInOwl:id>
        <rdfs:label>Palotai-sziget</rdfs:label>
    </owl:NamedIndividual>
    


    <!-- http://purl.obolibrary.org/obo/GAZ_00043963 -->

    <owl:NamedIndividual rdf:about="http://purl.obolibrary.org/obo/GAZ_00043963">
        <obo:RO_0001025 rdf:resource="http://purl.obolibrary.org/obo/GAZ_00003594"/>
        <obo:RO_0001025 rdf:resource="http://purl.obolibrary.org/obo/GAZ_00036861"/>
        <oboInOwl:hasOBONamespace>GAZ</oboInOwl:hasOBONamespace>
        <oboInOwl:id>GAZ:00043963</oboInOwl:id>
        <rdfs:label>Haros-sziget</rdfs:label>
    </owl:NamedIndividual>
    


    <!-- http://purl.obolibrary.org/obo/GAZ_00043964 -->

    <owl:NamedIndividual rdf:about="http://purl.obolibrary.org/obo/GAZ_00043964">
        <obo:RO_0001025 rdf:resource="http://purl.obolibrary.org/obo/GAZ_00003594"/>
        <obo:RO_0001025 rdf:resource="http://purl.obolibrary.org/obo/GAZ_00036861"/>
        <oboInOwl:hasOBONamespace>GAZ</oboInOwl:hasOBONamespace>
        <oboInOwl:id>GAZ:00043964</oboInOwl:id>
        <rdfs:label>Nep-sziget</rdfs:label>
    </owl:NamedIndividual>
    


    <!-- http://purl.obolibrary.org/obo/GAZ_00043965 -->

    <owl:NamedIndividual rdf:about="http://purl.obolibrary.org/obo/GAZ_00043965">
        <obo:RO_0001025 rdf:resource="http://purl.obolibrary.org/obo/GAZ_00007378"/>
    </owl:NamedIndividual>
    


    <!-- http://purl.obolibrary.org/obo/GAZ_00043966 -->

    <owl:NamedIndividual rdf:about="http://purl.obolibrary.org/obo/GAZ_00043966">
        <obo:RO_0001025 rdf:resource="http://purl.obolibrary.org/obo/GAZ_00003594"/>
        <obo:RO_0001025 rdf:resource="http://purl.obolibrary.org/obo/GAZ_00043965"/>
        <oboInOwl:hasOBONamespace>GAZ</oboInOwl:hasOBONamespace>
        <oboInOwl:id>GAZ:00043966</oboInOwl:id>
        <rdfs:label>Kortvelyesi-sziget</rdfs:label>
    </owl:NamedIndividual>
    


    <!-- http://purl.obolibrary.org/obo/GAZ_00043967 -->

    <owl:NamedIndividual rdf:about="http://purl.obolibrary.org/obo/GAZ_00043967">
        <obo:RO_0001025 rdf:resource="http://purl.obolibrary.org/obo/GAZ_00003594"/>
        <obo:RO_0001025 rdf:resource="http://purl.obolibrary.org/obo/GAZ_00043965"/>
        <oboInOwl:hasOBONamespace>GAZ</oboInOwl:hasOBONamespace>
        <oboInOwl:id>GAZ:00043967</oboInOwl:id>
        <rdfs:label>Nyaros-sziget</rdfs:label>
    </owl:NamedIndividual>
    


    <!-- http://purl.obolibrary.org/obo/GAZ_00043968 -->

    <owl:NamedIndividual rdf:about="http://purl.obolibrary.org/obo/GAZ_00043968">
        <obo:RO_0001025 rdf:resource="http://purl.obolibrary.org/obo/GAZ_00003594"/>
        <obo:RO_0001025 rdf:resource="http://purl.obolibrary.org/obo/GAZ_00043965"/>
        <oboInOwl:hasOBONamespace>GAZ</oboInOwl:hasOBONamespace>
        <oboInOwl:id>GAZ:00043968</oboInOwl:id>
        <rdfs:label>Torpe-sziget</rdfs:label>
    </owl:NamedIndividual>
    


    <!-- http://purl.obolibrary.org/obo/GAZ_00043969 -->

    <owl:NamedIndividual rdf:about="http://purl.obolibrary.org/obo/GAZ_00043969">
        <obo:RO_0001025 rdf:resource="http://purl.obolibrary.org/obo/GAZ_00003594"/>
        <obo:RO_0001025 rdf:resource="http://purl.obolibrary.org/obo/GAZ_00043965"/>
        <oboInOwl:hasOBONamespace>GAZ</oboInOwl:hasOBONamespace>
        <oboInOwl:id>GAZ:00043969</oboInOwl:id>
        <rdfs:label>Csitri-sziget</rdfs:label>
    </owl:NamedIndividual>
    


    <!-- http://purl.obolibrary.org/obo/GAZ_00043970 -->

    <owl:NamedIndividual rdf:about="http://purl.obolibrary.org/obo/GAZ_00043970">
        <obo:RO_0001025 rdf:resource="http://purl.obolibrary.org/obo/GAZ_00003594"/>
        <obo:RO_0001025 rdf:resource="http://purl.obolibrary.org/obo/GAZ_00043965"/>
        <oboInOwl:hasOBONamespace>GAZ</oboInOwl:hasOBONamespace>
        <oboInOwl:id>GAZ:00043970</oboInOwl:id>
        <rdfs:label>Helemba-sziget</rdfs:label>
    </owl:NamedIndividual>
    


    <!-- http://purl.obolibrary.org/obo/GAZ_00043971 -->

    <owl:NamedIndividual rdf:about="http://purl.obolibrary.org/obo/GAZ_00043971">
        <obo:RO_0001025 rdf:resource="http://purl.obolibrary.org/obo/GAZ_00003594"/>
        <obo:RO_0001025 rdf:resource="http://purl.obolibrary.org/obo/GAZ_00043965"/>
        <oboInOwl:hasOBONamespace>GAZ</oboInOwl:hasOBONamespace>
        <oboInOwl:id>GAZ:00043971</oboInOwl:id>
        <rdfs:label>Primas-sziget</rdfs:label>
    </owl:NamedIndividual>
    


    <!-- http://purl.obolibrary.org/obo/GAZ_00043972 -->

    <owl:NamedIndividual rdf:about="http://purl.obolibrary.org/obo/GAZ_00043972">
        <obo:RO_0001025 rdf:resource="http://purl.obolibrary.org/obo/GAZ_00003594"/>
        <obo:RO_0001025 rdf:resource="http://purl.obolibrary.org/obo/GAZ_00043965"/>
        <oboInOwl:hasOBONamespace>GAZ</oboInOwl:hasOBONamespace>
        <oboInOwl:id>GAZ:00043972</oboInOwl:id>
        <rdfs:label>Dedai-sziget</rdfs:label>
    </owl:NamedIndividual>
    


    <!-- http://purl.obolibrary.org/obo/GAZ_00056819 -->

    <owl:NamedIndividual rdf:about="http://purl.obolibrary.org/obo/GAZ_00056819">
        <obo:RO_0001025 rdf:resource="http://purl.obolibrary.org/obo/GAZ_00005067"/>
        <obo:IAO_0000115>A part of the European Tatra Mountains range in Poland and Slovakia. The Eastern Tatras consist of the High Tatras and the Belianske Tatras ranges.</obo:IAO_0000115>
        <oboInOwl:hasOBONamespace>GAZ</oboInOwl:hasOBONamespace>
        <oboInOwl:id>GAZ:00056819</oboInOwl:id>
        <rdfs:label>Eastern Tatras</rdfs:label>
    </owl:NamedIndividual>
    


    <!-- http://purl.obolibrary.org/obo/GAZ_00056820 -->

    <owl:NamedIndividual rdf:about="http://purl.obolibrary.org/obo/GAZ_00056820">
        <obo:RO_0001025 rdf:resource="http://purl.obolibrary.org/obo/GAZ_00005067"/>
        <obo:IAO_0000115>A mountain range in the Tatras, part of the Carpathian Mountains, located on the Polish-Slovak borders. The mountains border the High Tatras in the east. In Slovakia, they are partially located in the traditional regions of Liptov and Orava.</obo:IAO_0000115>
        <oboInOwl:hasOBONamespace>GAZ</oboInOwl:hasOBONamespace>
        <oboInOwl:id>GAZ:00056820</oboInOwl:id>
        <rdfs:label>Western Tatras</rdfs:label>
    </owl:NamedIndividual>
    


    <!-- http://purl.obolibrary.org/obo/GAZ_00056821 -->

    <owl:NamedIndividual rdf:about="http://purl.obolibrary.org/obo/GAZ_00056821">
        <obo:RO_0001025 rdf:resource="http://purl.obolibrary.org/obo/GAZ_00056819"/>
        <obo:RO_0001025 rdf:resource="http://purl.obolibrary.org/obo/GAZ_00056822"/>
        <obo:IAO_0000115>A mountain range in the Eastern Tatras in North Central Slovakia. Eastern Tatras are part of the Tatra Mountains, which are part of the Carpathian Mountains.</obo:IAO_0000115>
        <oboInOwl:hasOBONamespace>GAZ</oboInOwl:hasOBONamespace>
        <oboInOwl:id>GAZ:00056821</oboInOwl:id>
        <rdfs:label>Belianske Tatras</rdfs:label>
    </owl:NamedIndividual>
    


    <!-- http://purl.obolibrary.org/obo/GAZ_00056822 -->

    <owl:NamedIndividual rdf:about="http://purl.obolibrary.org/obo/GAZ_00056822">
        <obo:RO_0001025 rdf:resource="http://purl.obolibrary.org/obo/GAZ_00056819"/>
        <obo:RO_0001025 rdf:resource="http://purl.obolibrary.org/obo/GAZ_00056820"/>
        <obo:IAO_0000115>A national park located in North Central Slovakia in the Tatra Mountains. The Tatra National Park protects the area of the Western Tatras and the Eastern Tatras. The west part of the Tatra National Park is situated in the Zilina Region and the east part in the Presov Region. The Tatra National Park is located in the area of the Western Tatras (ZApadne Tatry) and the Eastern Tatras (Vychodne Tatry). The Western Tatras are divided into Osobita, Rohace, Sivy vrch, Liptovske Tatry (Liptov Tatras), Liptovske Kopy, Cervene vrchy. The Eastern Tatras consist of High Tatras (Vysoke Tatry) and Belianske Tatras (Belianske Tatry).</obo:IAO_0000115>
        <oboInOwl:hasOBONamespace>GAZ</oboInOwl:hasOBONamespace>
        <oboInOwl:id>GAZ:00056822</oboInOwl:id>
        <rdfs:label>Tatra National Park [Slovakia]</rdfs:label>
    </owl:NamedIndividual>
    


    <!-- http://purl.obolibrary.org/obo/GAZ_00056823 -->

    <owl:NamedIndividual rdf:about="http://purl.obolibrary.org/obo/GAZ_00056823">
        <obo:RO_0001025 rdf:resource="http://purl.obolibrary.org/obo/GAZ_00061695"/>
        <obo:IAO_0000115>A series of mountain ranges in the northeastern Czech Republic, northwestern Slovakia, southern Poland and in Western Ukraine. The Beskids are approximately 600 km in length and 50-70 km in width. They begin in Moravia at the Moravian Gate, continue to the north of the Tatra Mountains and end in Ukraine. The eastern border of the Beskids is disputed: according to older sources it is the sources of the Tisza River, according to newer sources the Beskids end at the Ushok Pass at the Polish-Ukrainian border.</obo:IAO_0000115>
        <oboInOwl:hasOBONamespace>GAZ</oboInOwl:hasOBONamespace>
        <oboInOwl:id>GAZ:00056823</oboInOwl:id>
        <rdfs:label>Beskidy Mountains</rdfs:label>
    </owl:NamedIndividual>
    


    <!-- http://purl.obolibrary.org/obo/GAZ_00058541 -->

    <owl:NamedIndividual rdf:about="http://purl.obolibrary.org/obo/GAZ_00058541">
        <obo:IAO_0000115>A lake in the Carpathian Mountains of Ukraine.</obo:IAO_0000115>
        <oboInOwl:hasOBONamespace>GAZ</oboInOwl:hasOBONamespace>
        <oboInOwl:id>GAZ:00058541</oboInOwl:id>
        <rdfs:label>Synevir Lake</rdfs:label>
    </owl:NamedIndividual>
    


    <!-- http://purl.obolibrary.org/obo/GAZ_00058633 -->

    <owl:NamedIndividual rdf:about="http://purl.obolibrary.org/obo/GAZ_00058633">
        <obo:RO_0001025 rdf:resource="http://purl.obolibrary.org/obo/GAZ_00088604"/>
        <obo:RO_0001025 rdf:resource="http://purl.obolibrary.org/obo/GAZ_00089829"/>
        <obo:IAO_0000115>An endorheic steppe lake straddling the border of Austria and Hungary.</obo:IAO_0000115>
        <oboInOwl:hasOBONamespace>GAZ</oboInOwl:hasOBONamespace>
        <oboInOwl:id>GAZ:00058633</oboInOwl:id>
        <rdfs:label>Neusiedlersee</rdfs:label>
    </owl:NamedIndividual>
    


    <!-- http://purl.obolibrary.org/obo/GAZ_00058983 -->

    <owl:NamedIndividual rdf:about="http://purl.obolibrary.org/obo/GAZ_00058983">
        <obo:RO_0001025 rdf:resource="http://purl.obolibrary.org/obo/GAZ_00002952"/>
        <obo:IAO_0000115>A lake in Hungary.</obo:IAO_0000115>
        <oboInOwl:hasOBONamespace>GAZ</oboInOwl:hasOBONamespace>
        <oboInOwl:id>GAZ:00058983</oboInOwl:id>
        <rdfs:label>Velencei-to</rdfs:label>
    </owl:NamedIndividual>
    


    <!-- http://purl.obolibrary.org/obo/GAZ_00059092 -->

    <owl:NamedIndividual rdf:about="http://purl.obolibrary.org/obo/GAZ_00059092">
        <obo:IAO_0000115>An artificial lake in central Bosnia and Herzegovina. It was created in 1953 when a hydroelectric dam was built to generate electricity.</obo:IAO_0000115>
        <oboInOwl:hasOBONamespace>GAZ</oboInOwl:hasOBONamespace>
        <oboInOwl:id>GAZ:00059092</oboInOwl:id>
        <rdfs:label>Jablanica Lake</rdfs:label>
    </owl:NamedIndividual>
    


    <!-- http://purl.obolibrary.org/obo/GAZ_00059133 -->

    <owl:NamedIndividual rdf:about="http://purl.obolibrary.org/obo/GAZ_00059133">
        <obo:IAO_0000115>An artificial lake in western Bulgaria, at the end of the Pancharevo Gorge of the Iskar River, located at 600 m above sea level between the Vitosha and Lozenska planina mountains. It is 3 km long and up to 700 m wide, reaching a depth of 30 m, and is situated 15 km southeast of the capital city of Sofia, where the Vitoshka Bistritsa flows into the Iskar. The villages of Pancharevo and Kokalyane and the Pancharevo mineral springs lie on the lake&apos;s western shore, while at the southern end of the lake there is a hydroelectric power station.</obo:IAO_0000115>
        <oboInOwl:hasOBONamespace>GAZ</oboInOwl:hasOBONamespace>
        <oboInOwl:id>GAZ:00059133</oboInOwl:id>
        <rdfs:label>Lake Pancharevo</rdfs:label>
    </owl:NamedIndividual>
    


    <!-- http://purl.obolibrary.org/obo/GAZ_00059134 -->

    <owl:NamedIndividual rdf:about="http://purl.obolibrary.org/obo/GAZ_00059134">
        <obo:IAO_0000115>A reservoir on the Iskar River. Constructed 1949-1954.</obo:IAO_0000115>
        <oboInOwl:hasOBONamespace>GAZ</oboInOwl:hasOBONamespace>
        <oboInOwl:id>GAZ:00059134</oboInOwl:id>
        <rdfs:label>Iskar Reservoir</rdfs:label>
    </owl:NamedIndividual>
    


    <!-- http://purl.obolibrary.org/obo/GAZ_00059135 -->

    <owl:NamedIndividual rdf:about="http://purl.obolibrary.org/obo/GAZ_00059135">
        <obo:IAO_0000115>A reservoir is located 20 km to the southeast of Sofia, Bulgaria at an altitude of 700 m. The dam is in the Iskar river, just downstream of Dolni Pasarel village.</obo:IAO_0000115>
        <oboInOwl:hasOBONamespace>GAZ</oboInOwl:hasOBONamespace>
        <oboInOwl:id>GAZ:00059135</oboInOwl:id>
        <rdfs:label>Pasarel Reservoir</rdfs:label>
    </owl:NamedIndividual>
    


    <!-- http://purl.obolibrary.org/obo/GAZ_00059147 -->

    <owl:NamedIndividual rdf:about="http://purl.obolibrary.org/obo/GAZ_00059147">
        <obo:IAO_0000115>A lake in the SW part of Zagreb, Croatia. It is formed by the Sava River.</obo:IAO_0000115>
        <oboInOwl:hasOBONamespace>GAZ</oboInOwl:hasOBONamespace>
        <oboInOwl:id>GAZ:00059147</oboInOwl:id>
        <rdfs:label>Jarun Lake</rdfs:label>
    </owl:NamedIndividual>
    


    <!-- http://purl.obolibrary.org/obo/GAZ_00059192 -->

    <owl:NamedIndividual rdf:about="http://purl.obolibrary.org/obo/GAZ_00059192">
        <obo:IAO_0000115>A reservoir.</obo:IAO_0000115>
        <oboInOwl:hasOBONamespace>GAZ</oboInOwl:hasOBONamespace>
        <oboInOwl:id>GAZ:00059192</oboInOwl:id>
        <rdfs:label>Vodni nadrz Dalesice</rdfs:label>
    </owl:NamedIndividual>
    


    <!-- http://purl.obolibrary.org/obo/GAZ_00061537 -->

    <owl:NamedIndividual rdf:about="http://purl.obolibrary.org/obo/GAZ_00061537">
        <obo:IAO_0000115>A populated place. A City district (Stadtteil).</obo:IAO_0000115>
        <oboInOwl:hasOBONamespace>GAZ</oboInOwl:hasOBONamespace>
        <oboInOwl:id>GAZ:00061537</oboInOwl:id>
        <rdfs:label>Eixendorftalsperre</rdfs:label>
    </owl:NamedIndividual>
    


    <!-- http://purl.obolibrary.org/obo/GAZ_00061553 -->

    <owl:NamedIndividual rdf:about="http://purl.obolibrary.org/obo/GAZ_00061553">
        <obo:IAO_0000115>A flood retention basin in Bavaria.</obo:IAO_0000115>
        <oboInOwl:hasOBONamespace>GAZ</oboInOwl:hasOBONamespace>
        <oboInOwl:id>GAZ:00061553</oboInOwl:id>
        <rdfs:label>Hochwasserspeicher Furth im Wald</rdfs:label>
    </owl:NamedIndividual>
    


    <!-- http://purl.obolibrary.org/obo/GAZ_00061664 -->

    <owl:NamedIndividual rdf:about="http://purl.obolibrary.org/obo/GAZ_00061664">
        <obo:RO_0001025 rdf:resource="http://purl.obolibrary.org/obo/GAZ_00014340"/>
        <obo:IAO_0000115>A thermal lake located in Heviz (Hungary), near to the western end of Lake Balaton, five miles from Keszthely.</obo:IAO_0000115>
        <oboInOwl:hasOBONamespace>GAZ</oboInOwl:hasOBONamespace>
        <oboInOwl:id>GAZ:00061664</oboInOwl:id>
        <rdfs:label>Lake Heviz</rdfs:label>
    </owl:NamedIndividual>
    


    <!-- http://purl.obolibrary.org/obo/GAZ_00061683 -->

    <owl:NamedIndividual rdf:about="http://purl.obolibrary.org/obo/GAZ_00061683">
        <obo:RO_0001025 rdf:resource="http://purl.obolibrary.org/obo/GAZ_00089824"/>
        <obo:IAO_0000115>A saline lake in Bacs-Kiskun county, Hungary. It is unusual salt lake formed from an old branch of the Danube, Lake Szelid can be found 4 km southeast from Dunapataj.</obo:IAO_0000115>
        <oboInOwl:hasOBONamespace>GAZ</oboInOwl:hasOBONamespace>
        <oboInOwl:id>GAZ:00061683</oboInOwl:id>
        <rdfs:label>Lake Szelid</rdfs:label>
    </owl:NamedIndividual>
    


    <!-- http://purl.obolibrary.org/obo/GAZ_00061684 -->

    <owl:NamedIndividual rdf:about="http://purl.obolibrary.org/obo/GAZ_00061684">
        <obo:RO_0001025 rdf:resource="http://purl.obolibrary.org/obo/GAZ_00014339"/>
        <obo:IAO_0000115>A reservoir located at the southeastern edge of Heves county, next to counties Borsod-Abaj-Zemplen, Hajde-Bihar and Jasz-Nagykun-Szolnok. As part of the ongoing Tisza River flood control project, it was built in 1973.</obo:IAO_0000115>
        <oboInOwl:hasOBONamespace>GAZ</oboInOwl:hasOBONamespace>
        <oboInOwl:id>GAZ:00061684</oboInOwl:id>
        <rdfs:label>Lake Tisza</rdfs:label>
    </owl:NamedIndividual>
    


    <!-- http://purl.obolibrary.org/obo/GAZ_00061685 -->

    <owl:NamedIndividual rdf:about="http://purl.obolibrary.org/obo/GAZ_00061685">
        <obo:RO_0001025 rdf:resource="http://purl.obolibrary.org/obo/GAZ_00089824"/>
        <obo:IAO_0000115>A freshwater lake nearby the town of Soltvadkert, Hungary.</obo:IAO_0000115>
        <oboInOwl:hasOBONamespace>GAZ</oboInOwl:hasOBONamespace>
        <oboInOwl:id>GAZ:00061685</oboInOwl:id>
        <rdfs:label>Lake Vadkert</rdfs:label>
    </owl:NamedIndividual>
    


    <!-- http://purl.obolibrary.org/obo/GAZ_00061686 -->

    <owl:NamedIndividual rdf:about="http://purl.obolibrary.org/obo/GAZ_00061686">
        <obo:RO_0001025 rdf:resource="http://purl.obolibrary.org/obo/GAZ_00014343"/>
        <obo:IAO_0000115>A lake located in Fejer county, on the motorway between Budapest and Szekesfeherver, at the feet of Velence Mountains.</obo:IAO_0000115>
        <oboInOwl:hasOBONamespace>GAZ</oboInOwl:hasOBONamespace>
        <oboInOwl:id>GAZ:00061686</oboInOwl:id>
        <rdfs:label>Lake Velence</rdfs:label>
    </owl:NamedIndividual>
    


    <!-- http://purl.obolibrary.org/obo/GAZ_00061687 -->

    <owl:NamedIndividual rdf:about="http://purl.obolibrary.org/obo/GAZ_00061687">
        <obo:RO_0001025 rdf:resource="http://purl.obolibrary.org/obo/GAZ_00002952"/>
        <obo:IAO_0000115>A mountain range in the Alpokalja area. The territory of the range is shared between Austria and Hungary.</obo:IAO_0000115>
        <oboInOwl:hasOBONamespace>GAZ</oboInOwl:hasOBONamespace>
        <oboInOwl:id>GAZ:00061687</oboInOwl:id>
        <rdfs:label>Koszeg Mountains</rdfs:label>
    </owl:NamedIndividual>
    


    <!-- http://purl.obolibrary.org/obo/GAZ_00061688 -->

    <owl:NamedIndividual rdf:about="http://purl.obolibrary.org/obo/GAZ_00061688">
        <obo:RO_0001025 rdf:resource="http://purl.obolibrary.org/obo/GAZ_00002952"/>
        <obo:IAO_0000115>A mountain range, the eastward extension of the Eastern Alps. It is part of the Alpokalja area of Hungary. It is located close to the city of Sopron (Western Hungary).</obo:IAO_0000115>
        <oboInOwl:hasOBONamespace>GAZ</oboInOwl:hasOBONamespace>
        <oboInOwl:id>GAZ:00061688</oboInOwl:id>
        <rdfs:label>Sopron Mountains</rdfs:label>
    </owl:NamedIndividual>
    


    <!-- http://purl.obolibrary.org/obo/GAZ_00061689 -->

    <owl:NamedIndividual rdf:about="http://purl.obolibrary.org/obo/GAZ_00061689">
        <obo:RO_0001025 rdf:resource="http://purl.obolibrary.org/obo/GAZ_00002952"/>
        <obo:RO_0001025 rdf:resource="http://purl.obolibrary.org/obo/GAZ_00061694"/>
        <obo:IAO_0000115>The northern, mountainous part of Hungary. It is forming a geographical unity with the Matra-Slanec Area, the adjacent parts of Slovakia. It is a separate geomorphological area within the Western Carpathians. The mountains run along in Norteast Hungary, and along the eastern parts of the Hungarian-Slovak border in a broad band from the Danube Bend to the town of Presov.</obo:IAO_0000115>
        <oboInOwl:hasOBONamespace>GAZ</oboInOwl:hasOBONamespace>
        <oboInOwl:id>GAZ:00061689</oboInOwl:id>
        <rdfs:label>Northern Medium Mountains</rdfs:label>
    </owl:NamedIndividual>
    


    <!-- http://purl.obolibrary.org/obo/GAZ_00061691 -->

    <owl:NamedIndividual rdf:about="http://purl.obolibrary.org/obo/GAZ_00061691">
        <obo:RO_0001025 rdf:resource="http://purl.obolibrary.org/obo/GAZ_00061689"/>
        <obo:IAO_0000115>A mountain range in Slovakia.</obo:IAO_0000115>
        <oboInOwl:hasOBONamespace>GAZ</oboInOwl:hasOBONamespace>
        <oboInOwl:id>GAZ:00061691</oboInOwl:id>
        <rdfs:label>Zemplin Mountains</rdfs:label>
    </owl:NamedIndividual>
    


    <!-- http://purl.obolibrary.org/obo/GAZ_00061692 -->

    <owl:NamedIndividual rdf:about="http://purl.obolibrary.org/obo/GAZ_00061692">
        <obo:RO_0001025 rdf:resource="http://purl.obolibrary.org/obo/GAZ_00061689"/>
        <obo:IAO_0000115>A mountain range in Slovakia.</obo:IAO_0000115>
        <oboInOwl:hasOBONamespace>GAZ</oboInOwl:hasOBONamespace>
        <oboInOwl:id>GAZ:00061692</oboInOwl:id>
        <rdfs:label>Slanec Mountains</rdfs:label>
    </owl:NamedIndividual>
    


    <!-- http://purl.obolibrary.org/obo/GAZ_00061693 -->

    <owl:NamedIndividual rdf:about="http://purl.obolibrary.org/obo/GAZ_00061693">
        <rdf:type rdf:resource="http://purl.obolibrary.org/obo/ENVO_00000104"/>
        <obo:IAO_0000115>A province of the Carpathian Mountains.</obo:IAO_0000115>
        <oboInOwl:hasOBONamespace>GAZ</oboInOwl:hasOBONamespace>
        <oboInOwl:id>GAZ:00061693</oboInOwl:id>
        <rdfs:label>Western Carpathian Mountains</rdfs:label>
    </owl:NamedIndividual>
    


    <!-- http://purl.obolibrary.org/obo/GAZ_00061694 -->

    <owl:NamedIndividual rdf:about="http://purl.obolibrary.org/obo/GAZ_00061694">
        <obo:RO_0001025 rdf:resource="http://purl.obolibrary.org/obo/GAZ_00061693"/>
        <obo:IAO_0000115>A subprovince of the Carpathian Mountains.</obo:IAO_0000115>
        <oboInOwl:hasOBONamespace>GAZ</oboInOwl:hasOBONamespace>
        <oboInOwl:id>GAZ:00061694</oboInOwl:id>
        <rdfs:label>Inner Western Carpathian Mountains</rdfs:label>
    </owl:NamedIndividual>
    


    <!-- http://purl.obolibrary.org/obo/GAZ_00061695 -->

    <owl:NamedIndividual rdf:about="http://purl.obolibrary.org/obo/GAZ_00061695">
        <obo:RO_0001025 rdf:resource="http://purl.obolibrary.org/obo/GAZ_00061693"/>
        <obo:IAO_0000115>A subprovince of the Carpathian Mountains.</obo:IAO_0000115>
        <oboInOwl:hasOBONamespace>GAZ</oboInOwl:hasOBONamespace>
        <oboInOwl:id>GAZ:00061695</oboInOwl:id>
        <rdfs:label>Outer Western Carpathian Mountains</rdfs:label>
    </owl:NamedIndividual>
    


    <!-- http://purl.obolibrary.org/obo/GAZ_00061696 -->

    <owl:NamedIndividual rdf:about="http://purl.obolibrary.org/obo/GAZ_00061696">
        <oboInOwl:hasOBONamespace>GAZ</oboInOwl:hasOBONamespace>
        <oboInOwl:id>GAZ:00061696</oboInOwl:id>
        <rdfs:label>Southeastern Carpathian Mountains</rdfs:label>
    </owl:NamedIndividual>
    


    <!-- http://purl.obolibrary.org/obo/GAZ_00061697 -->

    <owl:NamedIndividual rdf:about="http://purl.obolibrary.org/obo/GAZ_00061697">
        <obo:IAO_0000115>A province of the Carpathian Mountains. A group of mountain ranges which divide central and southern Romania. They cover part of the Carpathian Mountains that is located between the Prahova River in the east and the Timis and Cerna Rivers in the west.</obo:IAO_0000115>
        <oboInOwl:hasOBONamespace>GAZ</oboInOwl:hasOBONamespace>
        <oboInOwl:id>GAZ:00061697</oboInOwl:id>
        <rdfs:label>Southern Carpathian Mountains</rdfs:label>
    </owl:NamedIndividual>
    


    <!-- http://purl.obolibrary.org/obo/GAZ_00061698 -->

    <owl:NamedIndividual rdf:about="http://purl.obolibrary.org/obo/GAZ_00061698">
        <obo:RO_0001025 rdf:resource="http://purl.obolibrary.org/obo/GAZ_00061696"/>
        <oboInOwl:hasOBONamespace>GAZ</oboInOwl:hasOBONamespace>
        <oboInOwl:id>GAZ:00061698</oboInOwl:id>
        <rdfs:label>Eastern Carpathian Mountains</rdfs:label>
    </owl:NamedIndividual>
    


    <!-- http://purl.obolibrary.org/obo/GAZ_00061699 -->

    <owl:NamedIndividual rdf:about="http://purl.obolibrary.org/obo/GAZ_00061699">
        <obo:IAO_0000115>A plateau in central Romania almost entirely surrounded by the Eastern, Southern and Romanian Western branches of the Carpathian Mountains.</obo:IAO_0000115>
        <oboInOwl:hasOBONamespace>GAZ</oboInOwl:hasOBONamespace>
        <oboInOwl:id>GAZ:00061699</oboInOwl:id>
        <rdfs:label>Transylvanian Plateau</rdfs:label>
    </owl:NamedIndividual>
    


    <!-- http://purl.obolibrary.org/obo/GAZ_00061700 -->

    <owl:NamedIndividual rdf:about="http://purl.obolibrary.org/obo/GAZ_00061700">
        <rdf:type rdf:resource="http://purl.obolibrary.org/obo/ENVO_00000104"/>
        <obo:RO_0001025 rdf:resource="http://purl.obolibrary.org/obo/GAZ_00061693"/>
        <obo:IAO_0000115>A province of the Carpathian Mountains.</obo:IAO_0000115>
        <oboInOwl:hasOBONamespace>GAZ</oboInOwl:hasOBONamespace>
        <oboInOwl:id>GAZ:00061700</oboInOwl:id>
        <rdfs:label>Romanian Western Carpathian Mountains</rdfs:label>
    </owl:NamedIndividual>
    


    <!-- http://purl.obolibrary.org/obo/GAZ_00061701 -->

    <owl:NamedIndividual rdf:about="http://purl.obolibrary.org/obo/GAZ_00061701">
        <oboInOwl:hasOBONamespace>GAZ</oboInOwl:hasOBONamespace>
        <oboInOwl:id>GAZ:00061701</oboInOwl:id>
        <rdfs:label>Serbian Carpathians</rdfs:label>
    </owl:NamedIndividual>
    


    <!-- http://purl.obolibrary.org/obo/GAZ_00061702 -->

    <owl:NamedIndividual rdf:about="http://purl.obolibrary.org/obo/GAZ_00061702">
        <obo:RO_0001025 rdf:resource="http://purl.obolibrary.org/obo/GAZ_00061699"/>
        <oboInOwl:hasOBONamespace>GAZ</oboInOwl:hasOBONamespace>
        <oboInOwl:id>GAZ:00061702</oboInOwl:id>
        <rdfs:label>Mures-Turda Depression</rdfs:label>
    </owl:NamedIndividual>
    


    <!-- http://purl.obolibrary.org/obo/GAZ_00061703 -->

    <owl:NamedIndividual rdf:about="http://purl.obolibrary.org/obo/GAZ_00061703">
        <obo:RO_0001025 rdf:resource="http://purl.obolibrary.org/obo/GAZ_00061699"/>
        <oboInOwl:hasOBONamespace>GAZ</oboInOwl:hasOBONamespace>
        <oboInOwl:id>GAZ:00061703</oboInOwl:id>
        <rdfs:label>Fagaras Depression</rdfs:label>
    </owl:NamedIndividual>
    


    <!-- http://purl.obolibrary.org/obo/GAZ_00061704 -->

    <owl:NamedIndividual rdf:about="http://purl.obolibrary.org/obo/GAZ_00061704">
        <obo:RO_0001025 rdf:resource="http://purl.obolibrary.org/obo/GAZ_00061699"/>
        <oboInOwl:hasOBONamespace>GAZ</oboInOwl:hasOBONamespace>
        <oboInOwl:id>GAZ:00061704</oboInOwl:id>
        <rdfs:label>Sibiu Depression</rdfs:label>
    </owl:NamedIndividual>
    


    <!-- http://purl.obolibrary.org/obo/GAZ_00061705 -->

    <owl:NamedIndividual rdf:about="http://purl.obolibrary.org/obo/GAZ_00061705">
        <obo:RO_0001025 rdf:resource="http://purl.obolibrary.org/obo/GAZ_00061700"/>
        <obo:IAO_0000115>A mountain range in Transylvania, Romania, which belongs to the Western Carpathians. It boundaries are: N, the Barcau River; S, the Mures River.</obo:IAO_0000115>
        <oboInOwl:hasOBONamespace>GAZ</oboInOwl:hasOBONamespace>
        <oboInOwl:id>GAZ:00061705</oboInOwl:id>
        <rdfs:label>Apuseni Mountains</rdfs:label>
    </owl:NamedIndividual>
    


    <!-- http://purl.obolibrary.org/obo/GAZ_00061706 -->

    <owl:NamedIndividual rdf:about="http://purl.obolibrary.org/obo/GAZ_00061706">
        <obo:RO_0001025 rdf:resource="http://purl.obolibrary.org/obo/GAZ_00061700"/>
        <oboInOwl:hasOBONamespace>GAZ</oboInOwl:hasOBONamespace>
        <oboInOwl:id>GAZ:00061706</oboInOwl:id>
        <rdfs:label>Banat Mountain Range</rdfs:label>
    </owl:NamedIndividual>
    


    <!-- http://purl.obolibrary.org/obo/GAZ_00061707 -->

    <owl:NamedIndividual rdf:about="http://purl.obolibrary.org/obo/GAZ_00061707">
        <obo:RO_0001025 rdf:resource="http://purl.obolibrary.org/obo/GAZ_00062029"/>
        <oboInOwl:hasOBONamespace>GAZ</oboInOwl:hasOBONamespace>
        <oboInOwl:id>GAZ:00061707</oboInOwl:id>
        <rdfs:label>Hateg Depression</rdfs:label>
    </owl:NamedIndividual>
    


    <!-- http://purl.obolibrary.org/obo/GAZ_00061708 -->

    <owl:NamedIndividual rdf:about="http://purl.obolibrary.org/obo/GAZ_00061708">
        <obo:RO_0001025 rdf:resource="http://purl.obolibrary.org/obo/GAZ_00061697"/>
        <obo:IAO_0000115>A subgroup of mountains in the Southern Carpathians. Its borders are: W, the Olt River; E the Rucar-Bran gap and the Dambovita River.</obo:IAO_0000115>
        <oboInOwl:hasOBONamespace>GAZ</oboInOwl:hasOBONamespace>
        <oboInOwl:id>GAZ:00061708</oboInOwl:id>
        <rdfs:label>Fagaras Mountains Group</rdfs:label>
    </owl:NamedIndividual>
    


    <!-- http://purl.obolibrary.org/obo/GAZ_00061709 -->

    <owl:NamedIndividual rdf:about="http://purl.obolibrary.org/obo/GAZ_00061709">
        <obo:RO_0001025 rdf:resource="http://purl.obolibrary.org/obo/GAZ_00061697"/>
        <obo:IAO_0000115>A subgroup of mountains in the Southern Carpathians. Its borders are: E, the Olt River, W, the Jiu River.</obo:IAO_0000115>
        <oboInOwl:hasOBONamespace>GAZ</oboInOwl:hasOBONamespace>
        <oboInOwl:id>GAZ:00061709</oboInOwl:id>
        <rdfs:label>Parang Mountain Group</rdfs:label>
    </owl:NamedIndividual>
    


    <!-- http://purl.obolibrary.org/obo/GAZ_00061710 -->

    <owl:NamedIndividual rdf:about="http://purl.obolibrary.org/obo/GAZ_00061710">
        <obo:RO_0001025 rdf:resource="http://purl.obolibrary.org/obo/GAZ_00061697"/>
        <obo:IAO_0000115>A subgroup of mountains in the Southern Carpathians. Its borders are: E, Jiu River; W, the Timis-Cerna Gap (the Cerna River and the Timis River); N, the Bistra River and the Hateg depression.</obo:IAO_0000115>
        <oboInOwl:hasOBONamespace>GAZ</oboInOwl:hasOBONamespace>
        <oboInOwl:id>GAZ:00061710</oboInOwl:id>
        <rdfs:label>Retezat-Godeanu Mountain Group</rdfs:label>
    </owl:NamedIndividual>
    


    <!-- http://purl.obolibrary.org/obo/GAZ_00061711 -->

    <owl:NamedIndividual rdf:about="http://purl.obolibrary.org/obo/GAZ_00061711">
        <obo:RO_0001025 rdf:resource="http://purl.obolibrary.org/obo/GAZ_00061697"/>
        <obo:IAO_0000115>A subgroup of mountains in the Southern Carpathians. It lies between the Prahova and Dambovita Rivers.</obo:IAO_0000115>
        <oboInOwl:hasOBONamespace>GAZ</oboInOwl:hasOBONamespace>
        <oboInOwl:id>GAZ:00061711</oboInOwl:id>
        <rdfs:label>Bucegi Mountain Group</rdfs:label>
    </owl:NamedIndividual>
    


    <!-- http://purl.obolibrary.org/obo/GAZ_00061712 -->

    <owl:NamedIndividual rdf:about="http://purl.obolibrary.org/obo/GAZ_00061712">
        <obo:RO_0001025 rdf:resource="http://purl.obolibrary.org/obo/GAZ_00061693"/>
        <obo:IAO_0000115>A subprovince of the Carpathian Mountains.</obo:IAO_0000115>
        <oboInOwl:hasOBONamespace>GAZ</oboInOwl:hasOBONamespace>
        <oboInOwl:id>GAZ:00061712</oboInOwl:id>
        <rdfs:label>Outer Carpathian Depressions</rdfs:label>
    </owl:NamedIndividual>
    


    <!-- http://purl.obolibrary.org/obo/GAZ_00061713 -->

    <owl:NamedIndividual rdf:about="http://purl.obolibrary.org/obo/GAZ_00061713">
        <obo:RO_0001025 rdf:resource="http://purl.obolibrary.org/obo/GAZ_00061712"/>
        <obo:IAO_0000115>A division of the Outer Carpathian Depressions. A mountain range located in the northeast of Lower Austria. In the east, the Weinviertel borders Slovakia at the March (river). In the south, it borders Mostviertel and Industrieviertel, its limits being the Wagram, the Danube and the Marchfeld. Its western neighbor is Waldviertel, the traditional border being the Manhartsberg. In the north, the Weinviertel is adjacent to the Czech Republic, more specifically Moravia. The river Thaya runs back and forth across the border.</obo:IAO_0000115>
        <oboInOwl:hasOBONamespace>GAZ</oboInOwl:hasOBONamespace>
        <oboInOwl:id>GAZ:00061713</oboInOwl:id>
        <rdfs:label>Weinviertel Hills</rdfs:label>
    </owl:NamedIndividual>
    


    <!-- http://purl.obolibrary.org/obo/GAZ_00061714 -->

    <owl:NamedIndividual rdf:about="http://purl.obolibrary.org/obo/GAZ_00061714">
        <obo:RO_0001025 rdf:resource="http://purl.obolibrary.org/obo/GAZ_00061712"/>
        <obo:IAO_0000115>A division of the Outer Carpathian Depressions.</obo:IAO_0000115>
        <oboInOwl:hasOBONamespace>GAZ</oboInOwl:hasOBONamespace>
        <oboInOwl:id>GAZ:00061714</oboInOwl:id>
        <rdfs:label>Vyskov Gate</rdfs:label>
    </owl:NamedIndividual>
    


    <!-- http://purl.obolibrary.org/obo/GAZ_00061715 -->

    <owl:NamedIndividual rdf:about="http://purl.obolibrary.org/obo/GAZ_00061715">
        <obo:RO_0001025 rdf:resource="http://purl.obolibrary.org/obo/GAZ_00061712"/>
        <obo:IAO_0000115>A division of the Outer Carpathian Depressions.</obo:IAO_0000115>
        <oboInOwl:hasOBONamespace>GAZ</oboInOwl:hasOBONamespace>
        <oboInOwl:id>GAZ:00061715</oboInOwl:id>
        <rdfs:label>Upper Moravian Vale</rdfs:label>
    </owl:NamedIndividual>
    


    <!-- http://purl.obolibrary.org/obo/GAZ_00061716 -->

    <owl:NamedIndividual rdf:about="http://purl.obolibrary.org/obo/GAZ_00061716">
        <obo:RO_0001025 rdf:resource="http://purl.obolibrary.org/obo/GAZ_00061712"/>
        <obo:IAO_0000115>A geomorphological feature in Moravia, Czech Republic. It is formed by the depression between the Western Carpathians and the Eastern Sudetes. The drainage divide between the upper Odra and the Becva rivers runs through it. It stretches from Moravia towards Silesia north-eastward in the length of about 65 km. It is bordered by the confluence of the Olza and the Odra rivers in the north.</obo:IAO_0000115>
        <oboInOwl:hasOBONamespace>GAZ</oboInOwl:hasOBONamespace>
        <oboInOwl:id>GAZ:00061716</oboInOwl:id>
        <rdfs:label>Moravian Gate</rdfs:label>
    </owl:NamedIndividual>
    


    <!-- http://purl.obolibrary.org/obo/GAZ_00061717 -->

    <owl:NamedIndividual rdf:about="http://purl.obolibrary.org/obo/GAZ_00061717">
        <obo:RO_0001025 rdf:resource="http://purl.obolibrary.org/obo/GAZ_00061712"/>
        <obo:IAO_0000115>A division of the Outer Carpathian Depressions.</obo:IAO_0000115>
        <oboInOwl:hasOBONamespace>GAZ</oboInOwl:hasOBONamespace>
        <oboInOwl:id>GAZ:00061717</oboInOwl:id>
        <rdfs:label>Oswiecim Basin</rdfs:label>
    </owl:NamedIndividual>
    


    <!-- http://purl.obolibrary.org/obo/GAZ_00061718 -->

    <owl:NamedIndividual rdf:about="http://purl.obolibrary.org/obo/GAZ_00061718">
        <obo:RO_0001025 rdf:resource="http://purl.obolibrary.org/obo/GAZ_00061712"/>
        <obo:IAO_0000115>A division of the Outer Carpathian Depressions.</obo:IAO_0000115>
        <oboInOwl:hasOBONamespace>GAZ</oboInOwl:hasOBONamespace>
        <oboInOwl:id>GAZ:00061718</oboInOwl:id>
        <rdfs:label>Sandomierz Basin</rdfs:label>
    </owl:NamedIndividual>
    


    <!-- http://purl.obolibrary.org/obo/GAZ_00061719 -->

    <owl:NamedIndividual rdf:about="http://purl.obolibrary.org/obo/GAZ_00061719">
        <obo:RO_0001025 rdf:resource="http://purl.obolibrary.org/obo/GAZ_00061712"/>
        <obo:IAO_0000115>A division of the Outer Carpathian Depressions.</obo:IAO_0000115>
        <oboInOwl:hasOBONamespace>GAZ</oboInOwl:hasOBONamespace>
        <oboInOwl:id>GAZ:00061719</oboInOwl:id>
        <rdfs:label>Drohobych Highlands</rdfs:label>
    </owl:NamedIndividual>
    


    <!-- http://purl.obolibrary.org/obo/GAZ_00061720 -->

    <owl:NamedIndividual rdf:about="http://purl.obolibrary.org/obo/GAZ_00061720">
        <obo:RO_0001025 rdf:resource="http://purl.obolibrary.org/obo/GAZ_00061712"/>
        <obo:IAO_0000115>A division of the Outer Carpathian Depressions.</obo:IAO_0000115>
        <oboInOwl:hasOBONamespace>GAZ</oboInOwl:hasOBONamespace>
        <oboInOwl:id>GAZ:00061720</oboInOwl:id>
        <rdfs:label>Dniester Plain</rdfs:label>
    </owl:NamedIndividual>
    


    <!-- http://purl.obolibrary.org/obo/GAZ_00061721 -->

    <owl:NamedIndividual rdf:about="http://purl.obolibrary.org/obo/GAZ_00061721">
        <obo:RO_0001025 rdf:resource="http://purl.obolibrary.org/obo/GAZ_00061712"/>
        <obo:IAO_0000115>A division of the Outer Carpathian Depressions.</obo:IAO_0000115>
        <oboInOwl:hasOBONamespace>GAZ</oboInOwl:hasOBONamespace>
        <oboInOwl:id>GAZ:00061721</oboInOwl:id>
        <rdfs:label>Upper Dniester Plain</rdfs:label>
    </owl:NamedIndividual>
    


    <!-- http://purl.obolibrary.org/obo/GAZ_00061722 -->

    <owl:NamedIndividual rdf:about="http://purl.obolibrary.org/obo/GAZ_00061722">
        <obo:RO_0001025 rdf:resource="http://purl.obolibrary.org/obo/GAZ_00061712"/>
        <obo:IAO_0000115>A division of the Outer Carpathian Depressions.</obo:IAO_0000115>
        <oboInOwl:hasOBONamespace>GAZ</oboInOwl:hasOBONamespace>
        <oboInOwl:id>GAZ:00061722</oboInOwl:id>
        <rdfs:label>Ostrava Basin</rdfs:label>
    </owl:NamedIndividual>
    


    <!-- http://purl.obolibrary.org/obo/GAZ_00061723 -->

    <owl:NamedIndividual rdf:about="http://purl.obolibrary.org/obo/GAZ_00061723">
        <obo:RO_0001025 rdf:resource="http://purl.obolibrary.org/obo/GAZ_00061712"/>
        <obo:IAO_0000115>A division of the Outer Carpathian Depressions.</obo:IAO_0000115>
        <oboInOwl:hasOBONamespace>GAZ</oboInOwl:hasOBONamespace>
        <oboInOwl:id>GAZ:00061723</oboInOwl:id>
        <rdfs:label>Bucovina Highlands</rdfs:label>
    </owl:NamedIndividual>
    


    <!-- http://purl.obolibrary.org/obo/GAZ_00061724 -->

    <owl:NamedIndividual rdf:about="http://purl.obolibrary.org/obo/GAZ_00061724">
        <obo:RO_0001025 rdf:resource="http://purl.obolibrary.org/obo/GAZ_00061712"/>
        <obo:IAO_0000115>A division of the Outer Carpathian Depressions.</obo:IAO_0000115>
        <oboInOwl:hasOBONamespace>GAZ</oboInOwl:hasOBONamespace>
        <oboInOwl:id>GAZ:00061724</oboInOwl:id>
        <rdfs:label>Moldavian Subcarpathians</rdfs:label>
    </owl:NamedIndividual>
    


    <!-- http://purl.obolibrary.org/obo/GAZ_00061725 -->

    <owl:NamedIndividual rdf:about="http://purl.obolibrary.org/obo/GAZ_00061725">
        <obo:RO_0001025 rdf:resource="http://purl.obolibrary.org/obo/GAZ_00061712"/>
        <obo:IAO_0000115>A division of the Outer Carpathian Depressions.</obo:IAO_0000115>
        <oboInOwl:hasOBONamespace>GAZ</oboInOwl:hasOBONamespace>
        <oboInOwl:id>GAZ:00061725</oboInOwl:id>
        <rdfs:label>Pokutsk Upland</rdfs:label>
    </owl:NamedIndividual>
    


    <!-- http://purl.obolibrary.org/obo/GAZ_00061726 -->

    <owl:NamedIndividual rdf:about="http://purl.obolibrary.org/obo/GAZ_00061726">
        <obo:RO_0001025 rdf:resource="http://purl.obolibrary.org/obo/GAZ_00061712"/>
        <obo:IAO_0000115>A division of the Outer Carpathian Depressions.</obo:IAO_0000115>
        <oboInOwl:hasOBONamespace>GAZ</oboInOwl:hasOBONamespace>
        <oboInOwl:id>GAZ:00061726</oboInOwl:id>
        <rdfs:label>Muntenian Subcarpathians</rdfs:label>
    </owl:NamedIndividual>
    


    <!-- http://purl.obolibrary.org/obo/GAZ_00061727 -->

    <owl:NamedIndividual rdf:about="http://purl.obolibrary.org/obo/GAZ_00061727">
        <obo:RO_0001025 rdf:resource="http://purl.obolibrary.org/obo/GAZ_00061712"/>
        <obo:IAO_0000115>A division of the Outer Carpathian Depressions.</obo:IAO_0000115>
        <oboInOwl:hasOBONamespace>GAZ</oboInOwl:hasOBONamespace>
        <oboInOwl:id>GAZ:00061727</oboInOwl:id>
        <rdfs:label>Getic Plateau</rdfs:label>
    </owl:NamedIndividual>
    


    <!-- http://purl.obolibrary.org/obo/GAZ_00061728 -->

    <owl:NamedIndividual rdf:about="http://purl.obolibrary.org/obo/GAZ_00061728">
        <obo:RO_0001025 rdf:resource="http://purl.obolibrary.org/obo/GAZ_00061712"/>
        <obo:IAO_0000115>A division of the Outer Carpathian Depressions.</obo:IAO_0000115>
        <oboInOwl:hasOBONamespace>GAZ</oboInOwl:hasOBONamespace>
        <oboInOwl:id>GAZ:00061728</oboInOwl:id>
        <rdfs:label>Getic Subcarpathians</rdfs:label>
    </owl:NamedIndividual>
    


    <!-- http://purl.obolibrary.org/obo/GAZ_00061729 -->

    <owl:NamedIndividual rdf:about="http://purl.obolibrary.org/obo/GAZ_00061729">
        <obo:RO_0001025 rdf:resource="http://purl.obolibrary.org/obo/GAZ_00061712"/>
        <obo:IAO_0000115>A division of the Outer Carpathian Depressions.</obo:IAO_0000115>
        <oboInOwl:hasOBONamespace>GAZ</oboInOwl:hasOBONamespace>
        <oboInOwl:id>GAZ:00061729</oboInOwl:id>
        <rdfs:label>Moldavia-Siret Groove</rdfs:label>
    </owl:NamedIndividual>
    


    <!-- http://purl.obolibrary.org/obo/GAZ_00061730 -->

    <owl:NamedIndividual rdf:about="http://purl.obolibrary.org/obo/GAZ_00061730">
        <obo:RO_0001025 rdf:resource="http://purl.obolibrary.org/obo/GAZ_00061695"/>
        <obo:IAO_0000115>A division of the Outer Western Carpathian Mountains.</obo:IAO_0000115>
        <oboInOwl:hasOBONamespace>GAZ</oboInOwl:hasOBONamespace>
        <oboInOwl:id>GAZ:00061730</oboInOwl:id>
        <rdfs:label>South-Moravian Carpathians</rdfs:label>
    </owl:NamedIndividual>
    


    <!-- http://purl.obolibrary.org/obo/GAZ_00061731 -->

    <owl:NamedIndividual rdf:about="http://purl.obolibrary.org/obo/GAZ_00061731">
        <obo:RO_0001025 rdf:resource="http://purl.obolibrary.org/obo/GAZ_00061730"/>
        <oboInOwl:hasOBONamespace>GAZ</oboInOwl:hasOBONamespace>
        <oboInOwl:id>GAZ:00061731</oboInOwl:id>
        <rdfs:label>Mikulov Highlands</rdfs:label>
    </owl:NamedIndividual>
    


    <!-- http://purl.obolibrary.org/obo/GAZ_00061732 -->

    <owl:NamedIndividual rdf:about="http://purl.obolibrary.org/obo/GAZ_00061732">
        <obo:RO_0001025 rdf:resource="http://purl.obolibrary.org/obo/GAZ_00061730"/>
        <oboInOwl:hasOBONamespace>GAZ</oboInOwl:hasOBONamespace>
        <oboInOwl:id>GAZ:00061732</oboInOwl:id>
        <rdfs:label>Lower Austrian Inselberg Swell</rdfs:label>
    </owl:NamedIndividual>
    


    <!-- http://purl.obolibrary.org/obo/GAZ_00061733 -->

    <owl:NamedIndividual rdf:about="http://purl.obolibrary.org/obo/GAZ_00061733">
        <obo:RO_0001025 rdf:resource="http://purl.obolibrary.org/obo/GAZ_00061695"/>
        <obo:IAO_0000115>A division of the Outer Western Carpathian Mountains.</obo:IAO_0000115>
        <oboInOwl:hasOBONamespace>GAZ</oboInOwl:hasOBONamespace>
        <oboInOwl:id>GAZ:00061733</oboInOwl:id>
        <rdfs:label>Slovak-Moravian Carpathians</rdfs:label>
    </owl:NamedIndividual>
    


    <!-- http://purl.obolibrary.org/obo/GAZ_00061734 -->

    <owl:NamedIndividual rdf:about="http://purl.obolibrary.org/obo/GAZ_00061734">
        <obo:RO_0001025 rdf:resource="http://purl.obolibrary.org/obo/GAZ_00061695"/>
        <obo:IAO_0000115>A division of the Outer Western Carpathian Mountains.</obo:IAO_0000115>
        <oboInOwl:hasOBONamespace>GAZ</oboInOwl:hasOBONamespace>
        <oboInOwl:id>GAZ:00061734</oboInOwl:id>
        <rdfs:label>Central Moravian Carpathians</rdfs:label>
    </owl:NamedIndividual>
    


    <!-- http://purl.obolibrary.org/obo/GAZ_00061735 -->

    <owl:NamedIndividual rdf:about="http://purl.obolibrary.org/obo/GAZ_00061735">
        <obo:RO_0001025 rdf:resource="http://purl.obolibrary.org/obo/GAZ_00061734"/>
        <obo:IAO_0000115>A mountain range and forest in the Czech Republic, geologically part of the Central Moravian Carpathians of the Outer Western Carpathians.</obo:IAO_0000115>
        <oboInOwl:hasOBONamespace>GAZ</oboInOwl:hasOBONamespace>
        <oboInOwl:id>GAZ:00061735</oboInOwl:id>
        <rdfs:label>Zdanice Forest</rdfs:label>
    </owl:NamedIndividual>
    


    <!-- http://purl.obolibrary.org/obo/GAZ_00061736 -->

    <owl:NamedIndividual rdf:about="http://purl.obolibrary.org/obo/GAZ_00061736">
        <obo:RO_0001025 rdf:resource="http://purl.obolibrary.org/obo/GAZ_00061734"/>
        <oboInOwl:hasOBONamespace>GAZ</oboInOwl:hasOBONamespace>
        <oboInOwl:id>GAZ:00061736</oboInOwl:id>
        <rdfs:label>Litencice Hills</rdfs:label>
    </owl:NamedIndividual>
    


    <!-- http://purl.obolibrary.org/obo/GAZ_00061737 -->

    <owl:NamedIndividual rdf:about="http://purl.obolibrary.org/obo/GAZ_00061737">
        <obo:RO_0001025 rdf:resource="http://purl.obolibrary.org/obo/GAZ_00061734"/>
        <obo:IAO_0000115>A mountain range.</obo:IAO_0000115>
        <oboInOwl:hasOBONamespace>GAZ</oboInOwl:hasOBONamespace>
        <oboInOwl:id>GAZ:00061737</oboInOwl:id>
        <rdfs:label>Kyjov Hills</rdfs:label>
    </owl:NamedIndividual>
    


    <!-- http://purl.obolibrary.org/obo/GAZ_00061738 -->

    <owl:NamedIndividual rdf:about="http://purl.obolibrary.org/obo/GAZ_00061738">
        <obo:RO_0001025 rdf:resource="http://purl.obolibrary.org/obo/GAZ_00061734"/>
        <oboInOwl:hasOBONamespace>GAZ</oboInOwl:hasOBONamespace>
        <oboInOwl:id>GAZ:00061738</oboInOwl:id>
        <rdfs:label>Chriby</rdfs:label>
    </owl:NamedIndividual>
    


    <!-- http://purl.obolibrary.org/obo/GAZ_00061739 -->

    <owl:NamedIndividual rdf:about="http://purl.obolibrary.org/obo/GAZ_00061739">
        <obo:RO_0001025 rdf:resource="http://purl.obolibrary.org/obo/GAZ_00061733"/>
        <oboInOwl:hasOBONamespace>GAZ</oboInOwl:hasOBONamespace>
        <oboInOwl:id>GAZ:00061739</oboInOwl:id>
        <rdfs:label>Myjava Hills</rdfs:label>
    </owl:NamedIndividual>
    


    <!-- http://purl.obolibrary.org/obo/GAZ_00061740 -->

    <owl:NamedIndividual rdf:about="http://purl.obolibrary.org/obo/GAZ_00061740">
        <obo:RO_0001025 rdf:resource="http://purl.obolibrary.org/obo/GAZ_00061733"/>
        <obo:IAO_0000115>A mountain range of the western Carpathian Mountains that forms part of the border between the Czech Republic and Slovakia. The range divides the Becva-Oder river systems from those of the Turiec.</obo:IAO_0000115>
        <oboInOwl:hasOBONamespace>GAZ</oboInOwl:hasOBONamespace>
        <oboInOwl:id>GAZ:00061740</oboInOwl:id>
        <rdfs:label>Javorniky</rdfs:label>
    </owl:NamedIndividual>
    


    <!-- http://purl.obolibrary.org/obo/GAZ_00061741 -->

    <owl:NamedIndividual rdf:about="http://purl.obolibrary.org/obo/GAZ_00061741">
        <obo:RO_0001025 rdf:resource="http://purl.obolibrary.org/obo/GAZ_00061733"/>
        <oboInOwl:hasOBONamespace>GAZ</oboInOwl:hasOBONamespace>
        <oboInOwl:id>GAZ:00061741</oboInOwl:id>
        <rdfs:label>Vizovice Highlands</rdfs:label>
    </owl:NamedIndividual>
    


    <!-- http://purl.obolibrary.org/obo/GAZ_00061742 -->

    <owl:NamedIndividual rdf:about="http://purl.obolibrary.org/obo/GAZ_00061742">
        <obo:RO_0001025 rdf:resource="http://purl.obolibrary.org/obo/GAZ_00061733"/>
        <obo:IAO_0000115>The westernmost mountain range of the Carpathian Mountains. They are part of the Slovak-Moravian Carpathians and are situated on the border between the Czech Republic and Slovakia.</obo:IAO_0000115>
        <oboInOwl:hasOBONamespace>GAZ</oboInOwl:hasOBONamespace>
        <oboInOwl:id>GAZ:00061742</oboInOwl:id>
        <rdfs:label>White Carpathians</rdfs:label>
    </owl:NamedIndividual>
    


    <!-- http://purl.obolibrary.org/obo/GAZ_00061743 -->

    <owl:NamedIndividual rdf:about="http://purl.obolibrary.org/obo/GAZ_00061743">
        <obo:RO_0001025 rdf:resource="http://purl.obolibrary.org/obo/GAZ_00061733"/>
        <oboInOwl:hasOBONamespace>GAZ</oboInOwl:hasOBONamespace>
        <oboInOwl:id>GAZ:00061743</oboInOwl:id>
        <rdfs:label>Vah Valley Land</rdfs:label>
    </owl:NamedIndividual>
    


    <!-- http://purl.obolibrary.org/obo/GAZ_00061744 -->

    <owl:NamedIndividual rdf:about="http://purl.obolibrary.org/obo/GAZ_00061744">
        <obo:RO_0001025 rdf:resource="http://purl.obolibrary.org/obo/GAZ_00061695"/>
        <obo:IAO_0000115>A division of the Outer Western Carpathian Mountains.</obo:IAO_0000115>
        <oboInOwl:hasOBONamespace>GAZ</oboInOwl:hasOBONamespace>
        <oboInOwl:id>GAZ:00061744</oboInOwl:id>
        <rdfs:label>West-Beskidian Piedmont</rdfs:label>
    </owl:NamedIndividual>
    


    <!-- http://purl.obolibrary.org/obo/GAZ_00061745 -->

    <owl:NamedIndividual rdf:about="http://purl.obolibrary.org/obo/GAZ_00061745">
        <obo:RO_0001025 rdf:resource="http://purl.obolibrary.org/obo/GAZ_00061744"/>
        <oboInOwl:hasOBONamespace>GAZ</oboInOwl:hasOBONamespace>
        <oboInOwl:id>GAZ:00061745</oboInOwl:id>
        <rdfs:label>Moravian-Silesian Piedmont</rdfs:label>
    </owl:NamedIndividual>
    


    <!-- http://purl.obolibrary.org/obo/GAZ_00061746 -->

    <owl:NamedIndividual rdf:about="http://purl.obolibrary.org/obo/GAZ_00061746">
        <obo:RO_0001025 rdf:resource="http://purl.obolibrary.org/obo/GAZ_00061744"/>
        <oboInOwl:hasOBONamespace>GAZ</oboInOwl:hasOBONamespace>
        <oboInOwl:id>GAZ:00061746</oboInOwl:id>
        <rdfs:label>Silesian Piedmont</rdfs:label>
    </owl:NamedIndividual>
    


    <!-- http://purl.obolibrary.org/obo/GAZ_00061747 -->

    <owl:NamedIndividual rdf:about="http://purl.obolibrary.org/obo/GAZ_00061747">
        <obo:RO_0001025 rdf:resource="http://purl.obolibrary.org/obo/GAZ_00061744"/>
        <oboInOwl:hasOBONamespace>GAZ</oboInOwl:hasOBONamespace>
        <oboInOwl:id>GAZ:00061747</oboInOwl:id>
        <rdfs:label>Wieliczka Piedmont</rdfs:label>
    </owl:NamedIndividual>
    


    <!-- http://purl.obolibrary.org/obo/GAZ_00061748 -->

    <owl:NamedIndividual rdf:about="http://purl.obolibrary.org/obo/GAZ_00061748">
        <obo:RO_0001025 rdf:resource="http://purl.obolibrary.org/obo/GAZ_00061744"/>
        <oboInOwl:hasOBONamespace>GAZ</oboInOwl:hasOBONamespace>
        <oboInOwl:id>GAZ:00061748</oboInOwl:id>
        <rdfs:label>Wisnicz Piedmont</rdfs:label>
    </owl:NamedIndividual>
    


    <!-- http://purl.obolibrary.org/obo/GAZ_00061749 -->

    <owl:NamedIndividual rdf:about="http://purl.obolibrary.org/obo/GAZ_00061749">
        <obo:RO_0001025 rdf:resource="http://purl.obolibrary.org/obo/GAZ_00061744"/>
        <oboInOwl:hasOBONamespace>GAZ</oboInOwl:hasOBONamespace>
        <oboInOwl:id>GAZ:00061749</oboInOwl:id>
        <rdfs:label>Sub-Beskidian Hills</rdfs:label>
    </owl:NamedIndividual>
    


    <!-- http://purl.obolibrary.org/obo/GAZ_00061750 -->

    <owl:NamedIndividual rdf:about="http://purl.obolibrary.org/obo/GAZ_00061750">
        <obo:RO_0001025 rdf:resource="http://purl.obolibrary.org/obo/GAZ_00061695"/>
        <obo:IAO_0000115>A division of the Outer Western Carpathian Mountains.</obo:IAO_0000115>
        <oboInOwl:hasOBONamespace>GAZ</oboInOwl:hasOBONamespace>
        <oboInOwl:id>GAZ:00061750</oboInOwl:id>
        <rdfs:label>Podhale-Magura Area</rdfs:label>
    </owl:NamedIndividual>
    


    <!-- http://purl.obolibrary.org/obo/GAZ_00061751 -->

    <owl:NamedIndividual rdf:about="http://purl.obolibrary.org/obo/GAZ_00061751">
        <obo:RO_0001025 rdf:resource="http://purl.obolibrary.org/obo/GAZ_00056823"/>
        <obo:IAO_0000115>A division of the Outer Western Carpathian Mountains.</obo:IAO_0000115>
        <oboInOwl:hasOBONamespace>GAZ</oboInOwl:hasOBONamespace>
        <oboInOwl:id>GAZ:00061751</oboInOwl:id>
        <rdfs:label>Western Beskids</rdfs:label>
    </owl:NamedIndividual>
    


    <!-- http://purl.obolibrary.org/obo/GAZ_00061752 -->

    <owl:NamedIndividual rdf:about="http://purl.obolibrary.org/obo/GAZ_00061752">
        <obo:RO_0001025 rdf:resource="http://purl.obolibrary.org/obo/GAZ_00056823"/>
        <obo:IAO_0000115>A division of the Outer Western Carpathian Mountains.</obo:IAO_0000115>
        <oboInOwl:hasOBONamespace>GAZ</oboInOwl:hasOBONamespace>
        <oboInOwl:id>GAZ:00061752</oboInOwl:id>
        <rdfs:label>Eastern Beskids (Slovak)</rdfs:label>
    </owl:NamedIndividual>
    


    <!-- http://purl.obolibrary.org/obo/GAZ_00061753 -->

    <owl:NamedIndividual rdf:about="http://purl.obolibrary.org/obo/GAZ_00061753">
        <obo:RO_0001025 rdf:resource="http://purl.obolibrary.org/obo/GAZ_00056823"/>
        <obo:IAO_0000115>A division of the Outer Western Carpathian Mountains.</obo:IAO_0000115>
        <oboInOwl:hasOBONamespace>GAZ</oboInOwl:hasOBONamespace>
        <oboInOwl:id>GAZ:00061753</oboInOwl:id>
        <rdfs:label>Central Beskids</rdfs:label>
    </owl:NamedIndividual>
    


    <!-- http://purl.obolibrary.org/obo/GAZ_00061754 -->

    <owl:NamedIndividual rdf:about="http://purl.obolibrary.org/obo/GAZ_00061754">
        <obo:RO_0001025 rdf:resource="http://purl.obolibrary.org/obo/GAZ_00061751"/>
        <obo:IAO_0000115>A relatively flat and low mountain range in the Czech Republic. It is a part of the Western Carpathians, it is divided by the Beva River valley into the lower eastern Hostynske vrchy and the higher western Vsetinske vrchy which are a part of the Beskydy Landscape Protected Area.</obo:IAO_0000115>
        <oboInOwl:hasOBONamespace>GAZ</oboInOwl:hasOBONamespace>
        <oboInOwl:id>GAZ:00061754</oboInOwl:id>
        <rdfs:label>Hostynsko-vsetinska hornatina</rdfs:label>
    </owl:NamedIndividual>
    


    <!-- http://purl.obolibrary.org/obo/GAZ_00061755 -->

    <owl:NamedIndividual rdf:about="http://purl.obolibrary.org/obo/GAZ_00061755">
        <obo:RO_0001025 rdf:resource="http://purl.obolibrary.org/obo/GAZ_00061751"/>
        <obo:IAO_0000115>A mountain range in the Czech Republic with a small part reaching to Slovakia. It lies on the historical division between Moravia and Silesia, hence the name. In the south they slowly merge with the Javorniky. In the south-west they are separated from the Vsetinske vrchy by the Roznovska Becva valley, in the north-east the Jablunkov Pass separates them from the Silesian Beskids.</obo:IAO_0000115>
        <oboInOwl:hasOBONamespace>GAZ</oboInOwl:hasOBONamespace>
        <oboInOwl:id>GAZ:00061755</oboInOwl:id>
        <rdfs:label>Moravian-Silesian Beskids</rdfs:label>
    </owl:NamedIndividual>
    


    <!-- http://purl.obolibrary.org/obo/GAZ_00061756 -->

    <owl:NamedIndividual rdf:about="http://purl.obolibrary.org/obo/GAZ_00061756">
        <obo:RO_0001025 rdf:resource="http://purl.obolibrary.org/obo/GAZ_00061751"/>
        <obo:IAO_0000115>One of the Beskids mountain ranges in Outer Western Carpathians in southern Silesian Voivodeship, Poland and the eastern Czech Silesia Most of the range lies in Poland. It is separated from the Moravian-Silesian Beskids by the Jablunkov Pass.</obo:IAO_0000115>
        <oboInOwl:hasOBONamespace>GAZ</oboInOwl:hasOBONamespace>
        <oboInOwl:id>GAZ:00061756</oboInOwl:id>
        <rdfs:label>Silesian Beskids</rdfs:label>
    </owl:NamedIndividual>
    


    <!-- http://purl.obolibrary.org/obo/GAZ_00061757 -->

    <owl:NamedIndividual rdf:about="http://purl.obolibrary.org/obo/GAZ_00061757">
        <obo:RO_0001025 rdf:resource="http://purl.obolibrary.org/obo/GAZ_00061751"/>
        <oboInOwl:hasOBONamespace>GAZ</oboInOwl:hasOBONamespace>
        <oboInOwl:id>GAZ:00061757</oboInOwl:id>
        <rdfs:label>Zywiec Basin</rdfs:label>
    </owl:NamedIndividual>
    


    <!-- http://purl.obolibrary.org/obo/GAZ_00061758 -->

    <owl:NamedIndividual rdf:about="http://purl.obolibrary.org/obo/GAZ_00061758">
        <obo:RO_0001025 rdf:resource="http://purl.obolibrary.org/obo/GAZ_00061751"/>
        <oboInOwl:hasOBONamespace>GAZ</oboInOwl:hasOBONamespace>
        <oboInOwl:id>GAZ:00061758</oboInOwl:id>
        <rdfs:label>Jablunkov Furrow</rdfs:label>
    </owl:NamedIndividual>
    


    <!-- http://purl.obolibrary.org/obo/GAZ_00061759 -->

    <owl:NamedIndividual rdf:about="http://purl.obolibrary.org/obo/GAZ_00061759">
        <obo:RO_0001025 rdf:resource="http://purl.obolibrary.org/obo/GAZ_00061751"/>
        <oboInOwl:hasOBONamespace>GAZ</oboInOwl:hasOBONamespace>
        <oboInOwl:id>GAZ:00061759</oboInOwl:id>
        <rdfs:label>Jablunkov Intermontane</rdfs:label>
    </owl:NamedIndividual>
    


    <!-- http://purl.obolibrary.org/obo/GAZ_00061760 -->

    <owl:NamedIndividual rdf:about="http://purl.obolibrary.org/obo/GAZ_00061760">
        <obo:RO_0001025 rdf:resource="http://purl.obolibrary.org/obo/GAZ_00061751"/>
        <oboInOwl:hasOBONamespace>GAZ</oboInOwl:hasOBONamespace>
        <oboInOwl:id>GAZ:00061760</oboInOwl:id>
        <rdfs:label>Roznov Furrow</rdfs:label>
    </owl:NamedIndividual>
    


    <!-- http://purl.obolibrary.org/obo/GAZ_00061761 -->

    <owl:NamedIndividual rdf:about="http://purl.obolibrary.org/obo/GAZ_00061761">
        <obo:RO_0001025 rdf:resource="http://purl.obolibrary.org/obo/GAZ_00061751"/>
        <oboInOwl:hasOBONamespace>GAZ</oboInOwl:hasOBONamespace>
        <oboInOwl:id>GAZ:00061761</oboInOwl:id>
        <rdfs:label>Turzovka Highlands</rdfs:label>
    </owl:NamedIndividual>
    


    <!-- http://purl.obolibrary.org/obo/GAZ_00061762 -->

    <owl:NamedIndividual rdf:about="http://purl.obolibrary.org/obo/GAZ_00061762">
        <obo:RO_0001025 rdf:resource="http://purl.obolibrary.org/obo/GAZ_00061751"/>
        <obo:IAO_0000115>One of the Beskids mountain ranges in the Outer Western Carpathians in southeastern Poland.</obo:IAO_0000115>
        <oboInOwl:hasOBONamespace>GAZ</oboInOwl:hasOBONamespace>
        <oboInOwl:id>GAZ:00061762</oboInOwl:id>
        <rdfs:label>Little Beskids</rdfs:label>
    </owl:NamedIndividual>
    


    <!-- http://purl.obolibrary.org/obo/GAZ_00061763 -->

    <owl:NamedIndividual rdf:about="http://purl.obolibrary.org/obo/GAZ_00061763">
        <obo:RO_0001025 rdf:resource="http://purl.obolibrary.org/obo/GAZ_00061751"/>
        <obo:IAO_0000115>A mountain range.</obo:IAO_0000115>
        <oboInOwl:hasOBONamespace>GAZ</oboInOwl:hasOBONamespace>
        <oboInOwl:id>GAZ:00061763</oboInOwl:id>
        <rdfs:label>Gorce</rdfs:label>
    </owl:NamedIndividual>
    


    <!-- http://purl.obolibrary.org/obo/GAZ_00061764 -->

    <owl:NamedIndividual rdf:about="http://purl.obolibrary.org/obo/GAZ_00061764">
        <obo:RO_0001025 rdf:resource="http://purl.obolibrary.org/obo/GAZ_00061751"/>
        <oboInOwl:hasOBONamespace>GAZ</oboInOwl:hasOBONamespace>
        <oboInOwl:id>GAZ:00061764</oboInOwl:id>
        <rdfs:label>Makow Beskids</rdfs:label>
    </owl:NamedIndividual>
    


    <!-- http://purl.obolibrary.org/obo/GAZ_00061765 -->

    <owl:NamedIndividual rdf:about="http://purl.obolibrary.org/obo/GAZ_00061765">
        <obo:RO_0001025 rdf:resource="http://purl.obolibrary.org/obo/GAZ_00061751"/>
        <oboInOwl:hasOBONamespace>GAZ</oboInOwl:hasOBONamespace>
        <oboInOwl:id>GAZ:00061765</oboInOwl:id>
        <rdfs:label>Sacz Basin</rdfs:label>
    </owl:NamedIndividual>
    


    <!-- http://purl.obolibrary.org/obo/GAZ_00061766 -->

    <owl:NamedIndividual rdf:about="http://purl.obolibrary.org/obo/GAZ_00061766">
        <obo:RO_0001025 rdf:resource="http://purl.obolibrary.org/obo/GAZ_00061751"/>
        <oboInOwl:hasOBONamespace>GAZ</oboInOwl:hasOBONamespace>
        <oboInOwl:id>GAZ:00061766</oboInOwl:id>
        <rdfs:label>Rabka Basin</rdfs:label>
    </owl:NamedIndividual>
    


    <!-- http://purl.obolibrary.org/obo/GAZ_00061767 -->

    <owl:NamedIndividual rdf:about="http://purl.obolibrary.org/obo/GAZ_00061767">
        <obo:RO_0001025 rdf:resource="http://purl.obolibrary.org/obo/GAZ_00061751"/>
        <oboInOwl:hasOBONamespace>GAZ</oboInOwl:hasOBONamespace>
        <oboInOwl:id>GAZ:00061767</oboInOwl:id>
        <rdfs:label>Island Beskids</rdfs:label>
    </owl:NamedIndividual>
    


    <!-- http://purl.obolibrary.org/obo/GAZ_00061768 -->

    <owl:NamedIndividual rdf:about="http://purl.obolibrary.org/obo/GAZ_00061768">
        <obo:RO_0001025 rdf:resource="http://purl.obolibrary.org/obo/GAZ_00061752"/>
        <oboInOwl:hasOBONamespace>GAZ</oboInOwl:hasOBONamespace>
        <oboInOwl:id>GAZ:00061768</oboInOwl:id>
        <rdfs:label>Cergov</rdfs:label>
    </owl:NamedIndividual>
    


    <!-- http://purl.obolibrary.org/obo/GAZ_00061769 -->

    <owl:NamedIndividual rdf:about="http://purl.obolibrary.org/obo/GAZ_00061769">
        <obo:RO_0001025 rdf:resource="http://purl.obolibrary.org/obo/GAZ_00061752"/>
        <oboInOwl:hasOBONamespace>GAZ</oboInOwl:hasOBONamespace>
        <oboInOwl:id>GAZ:00061769</oboInOwl:id>
        <rdfs:label>Lubovna Highlands</rdfs:label>
    </owl:NamedIndividual>
    


    <!-- http://purl.obolibrary.org/obo/GAZ_00061770 -->

    <owl:NamedIndividual rdf:about="http://purl.obolibrary.org/obo/GAZ_00061770">
        <obo:RO_0001025 rdf:resource="http://purl.obolibrary.org/obo/GAZ_00061752"/>
        <oboInOwl:hasOBONamespace>GAZ</oboInOwl:hasOBONamespace>
        <oboInOwl:id>GAZ:00061770</oboInOwl:id>
        <rdfs:label>Czerchow Mountains</rdfs:label>
    </owl:NamedIndividual>
    


    <!-- http://purl.obolibrary.org/obo/GAZ_00061771 -->

    <owl:NamedIndividual rdf:about="http://purl.obolibrary.org/obo/GAZ_00061771">
        <obo:RO_0001025 rdf:resource="http://purl.obolibrary.org/obo/GAZ_00061752"/>
        <oboInOwl:hasOBONamespace>GAZ</oboInOwl:hasOBONamespace>
        <oboInOwl:id>GAZ:00061771</oboInOwl:id>
        <rdfs:label>Sacz Beskids</rdfs:label>
    </owl:NamedIndividual>
    


    <!-- http://purl.obolibrary.org/obo/GAZ_00061772 -->

    <owl:NamedIndividual rdf:about="http://purl.obolibrary.org/obo/GAZ_00061772">
        <obo:RO_0001025 rdf:resource="http://purl.obolibrary.org/obo/GAZ_00061752"/>
        <obo:IAO_0000115>A mountain range in Poland and Slovakia.</obo:IAO_0000115>
        <oboInOwl:hasOBONamespace>GAZ</oboInOwl:hasOBONamespace>
        <oboInOwl:id>GAZ:00061772</oboInOwl:id>
        <rdfs:label>Pieniny Mountains</rdfs:label>
    </owl:NamedIndividual>
    


    <!-- http://purl.obolibrary.org/obo/GAZ_00061773 -->

    <owl:NamedIndividual rdf:about="http://purl.obolibrary.org/obo/GAZ_00061773">
        <obo:RO_0001025 rdf:resource="http://purl.obolibrary.org/obo/GAZ_00061753"/>
        <obo:IAO_0000115>A mountain range in the Outer Eastern Carpathians in southern Poland.</obo:IAO_0000115>
        <oboInOwl:hasOBONamespace>GAZ</oboInOwl:hasOBONamespace>
        <oboInOwl:id>GAZ:00061773</oboInOwl:id>
        <rdfs:label>Zywiec Beskids</rdfs:label>
    </owl:NamedIndividual>
    


    <!-- http://purl.obolibrary.org/obo/GAZ_00061774 -->

    <owl:NamedIndividual rdf:about="http://purl.obolibrary.org/obo/GAZ_00061774">
        <obo:RO_0001025 rdf:resource="http://purl.obolibrary.org/obo/GAZ_00061753"/>
        <oboInOwl:hasOBONamespace>GAZ</oboInOwl:hasOBONamespace>
        <oboInOwl:id>GAZ:00061774</oboInOwl:id>
        <rdfs:label>Orava Magura</rdfs:label>
    </owl:NamedIndividual>
    


    <!-- http://purl.obolibrary.org/obo/GAZ_00061775 -->

    <owl:NamedIndividual rdf:about="http://purl.obolibrary.org/obo/GAZ_00061775">
        <obo:RO_0001025 rdf:resource="http://purl.obolibrary.org/obo/GAZ_00061753"/>
        <oboInOwl:hasOBONamespace>GAZ</oboInOwl:hasOBONamespace>
        <oboInOwl:id>GAZ:00061775</oboInOwl:id>
        <rdfs:label>Orava Highlands</rdfs:label>
    </owl:NamedIndividual>
    


    <!-- http://purl.obolibrary.org/obo/GAZ_00061776 -->

    <owl:NamedIndividual rdf:about="http://purl.obolibrary.org/obo/GAZ_00061776">
        <obo:RO_0001025 rdf:resource="http://purl.obolibrary.org/obo/GAZ_00061753"/>
        <oboInOwl:hasOBONamespace>GAZ</oboInOwl:hasOBONamespace>
        <oboInOwl:id>GAZ:00061776</oboInOwl:id>
        <rdfs:label>Sub-Beskidian Furrow</rdfs:label>
    </owl:NamedIndividual>
    


    <!-- http://purl.obolibrary.org/obo/GAZ_00061777 -->

    <owl:NamedIndividual rdf:about="http://purl.obolibrary.org/obo/GAZ_00061777">
        <rdf:type rdf:resource="http://purl.obolibrary.org/obo/ENVO_00000106"/>
        <obo:RO_0001025 rdf:resource="http://purl.obolibrary.org/obo/GAZ_00061753"/>
        <obo:IAO_0000115>A range of mountains straddling the northern-Slovakia-southern-Poland border, considered part of the Central Beskids, within the Outer Western Carpathians.</obo:IAO_0000115>
        <oboInOwl:hasOBONamespace>GAZ</oboInOwl:hasOBONamespace>
        <oboInOwl:id>GAZ:00061777</oboInOwl:id>
        <rdfs:label>Orava Beskids</rdfs:label>
    </owl:NamedIndividual>
    


    <!-- http://purl.obolibrary.org/obo/GAZ_00061778 -->

    <owl:NamedIndividual rdf:about="http://purl.obolibrary.org/obo/GAZ_00061778">
        <obo:RO_0001025 rdf:resource="http://purl.obolibrary.org/obo/GAZ_00061753"/>
        <oboInOwl:hasOBONamespace>GAZ</oboInOwl:hasOBONamespace>
        <oboInOwl:id>GAZ:00061778</oboInOwl:id>
        <rdfs:label>Kysuce Highlands</rdfs:label>
    </owl:NamedIndividual>
    


    <!-- http://purl.obolibrary.org/obo/GAZ_00061779 -->

    <owl:NamedIndividual rdf:about="http://purl.obolibrary.org/obo/GAZ_00061779">
        <obo:RO_0001025 rdf:resource="http://purl.obolibrary.org/obo/GAZ_00061753"/>
        <oboInOwl:hasOBONamespace>GAZ</oboInOwl:hasOBONamespace>
        <oboInOwl:id>GAZ:00061779</oboInOwl:id>
        <rdfs:label>Kysuce Beskids</rdfs:label>
    </owl:NamedIndividual>
    


    <!-- http://purl.obolibrary.org/obo/GAZ_00061780 -->

    <owl:NamedIndividual rdf:about="http://purl.obolibrary.org/obo/GAZ_00061780">
        <rdf:type rdf:resource="http://purl.obolibrary.org/obo/ENVO_00000106"/>
        <obo:RO_0001025 rdf:resource="http://purl.obolibrary.org/obo/GAZ_00061772"/>
        <obo:IAO_0000115>A Polish range of the Pieniny.</obo:IAO_0000115>
        <oboInOwl:hasOBONamespace>GAZ</oboInOwl:hasOBONamespace>
        <oboInOwl:id>GAZ:00061780</oboInOwl:id>
        <rdfs:label>Pieniny Spiskie</rdfs:label>
    </owl:NamedIndividual>
    


    <!-- http://purl.obolibrary.org/obo/GAZ_00061781 -->

    <owl:NamedIndividual rdf:about="http://purl.obolibrary.org/obo/GAZ_00061781">
        <obo:RO_0001025 rdf:resource="http://purl.obolibrary.org/obo/GAZ_00061753"/>
        <oboInOwl:hasOBONamespace>GAZ</oboInOwl:hasOBONamespace>
        <oboInOwl:id>GAZ:00061781</oboInOwl:id>
        <rdfs:label>Sub-Beskidian Highlands</rdfs:label>
    </owl:NamedIndividual>
    


    <!-- http://purl.obolibrary.org/obo/GAZ_00061782 -->

    <owl:NamedIndividual rdf:about="http://purl.obolibrary.org/obo/GAZ_00061782">
        <obo:RO_0001025 rdf:resource="http://purl.obolibrary.org/obo/GAZ_00061750"/>
        <oboInOwl:hasOBONamespace>GAZ</oboInOwl:hasOBONamespace>
        <oboInOwl:id>GAZ:00061782</oboInOwl:id>
        <rdfs:label>Orava-Nowy Targ Basin</rdfs:label>
    </owl:NamedIndividual>
    


    <!-- http://purl.obolibrary.org/obo/GAZ_00061783 -->

    <owl:NamedIndividual rdf:about="http://purl.obolibrary.org/obo/GAZ_00061783">
        <obo:RO_0001025 rdf:resource="http://purl.obolibrary.org/obo/GAZ_00061750"/>
        <oboInOwl:hasOBONamespace>GAZ</oboInOwl:hasOBONamespace>
        <oboInOwl:id>GAZ:00061783</oboInOwl:id>
        <rdfs:label>Saris Highlands</rdfs:label>
    </owl:NamedIndividual>
    


    <!-- http://purl.obolibrary.org/obo/GAZ_00061784 -->

    <owl:NamedIndividual rdf:about="http://purl.obolibrary.org/obo/GAZ_00061784">
        <obo:RO_0001025 rdf:resource="http://purl.obolibrary.org/obo/GAZ_00061750"/>
        <oboInOwl:hasOBONamespace>GAZ</oboInOwl:hasOBONamespace>
        <oboInOwl:id>GAZ:00061784</oboInOwl:id>
        <rdfs:label>Bachuren</rdfs:label>
    </owl:NamedIndividual>
    


    <!-- http://purl.obolibrary.org/obo/GAZ_00061785 -->

    <owl:NamedIndividual rdf:about="http://purl.obolibrary.org/obo/GAZ_00061785">
        <obo:RO_0001025 rdf:resource="http://purl.obolibrary.org/obo/GAZ_00061750"/>
        <oboInOwl:hasOBONamespace>GAZ</oboInOwl:hasOBONamespace>
        <oboInOwl:id>GAZ:00061785</oboInOwl:id>
        <rdfs:label>Spis Magura</rdfs:label>
    </owl:NamedIndividual>
    


    <!-- http://purl.obolibrary.org/obo/GAZ_00061786 -->

    <owl:NamedIndividual rdf:about="http://purl.obolibrary.org/obo/GAZ_00061786">
        <obo:RO_0001025 rdf:resource="http://purl.obolibrary.org/obo/GAZ_00061750"/>
        <oboInOwl:hasOBONamespace>GAZ</oboInOwl:hasOBONamespace>
        <oboInOwl:id>GAZ:00061786</oboInOwl:id>
        <rdfs:label>Orava Basin</rdfs:label>
    </owl:NamedIndividual>
    


    <!-- http://purl.obolibrary.org/obo/GAZ_00061787 -->

    <owl:NamedIndividual rdf:about="http://purl.obolibrary.org/obo/GAZ_00061787">
        <obo:RO_0001025 rdf:resource="http://purl.obolibrary.org/obo/GAZ_00061750"/>
        <oboInOwl:hasOBONamespace>GAZ</oboInOwl:hasOBONamespace>
        <oboInOwl:id>GAZ:00061787</oboInOwl:id>
        <rdfs:label>Levoca Mountains</rdfs:label>
    </owl:NamedIndividual>
    


    <!-- http://purl.obolibrary.org/obo/GAZ_00061788 -->

    <owl:NamedIndividual rdf:about="http://purl.obolibrary.org/obo/GAZ_00061788">
        <obo:RO_0001025 rdf:resource="http://purl.obolibrary.org/obo/GAZ_00061750"/>
        <oboInOwl:hasOBONamespace>GAZ</oboInOwl:hasOBONamespace>
        <oboInOwl:id>GAZ:00061788</oboInOwl:id>
        <rdfs:label>Skorusina Mountains</rdfs:label>
    </owl:NamedIndividual>
    


    <!-- http://purl.obolibrary.org/obo/GAZ_00061789 -->

    <owl:NamedIndividual rdf:about="http://purl.obolibrary.org/obo/GAZ_00061789">
        <obo:RO_0001025 rdf:resource="http://purl.obolibrary.org/obo/GAZ_00061750"/>
        <oboInOwl:hasOBONamespace>GAZ</oboInOwl:hasOBONamespace>
        <oboInOwl:id>GAZ:00061789</oboInOwl:id>
        <rdfs:label>Spis-Saris Intermontane</rdfs:label>
    </owl:NamedIndividual>
    


    <!-- http://purl.obolibrary.org/obo/GAZ_00061790 -->

    <owl:NamedIndividual rdf:about="http://purl.obolibrary.org/obo/GAZ_00061790">
        <obo:RO_0001025 rdf:resource="http://purl.obolibrary.org/obo/GAZ_00061750"/>
        <oboInOwl:hasOBONamespace>GAZ</oboInOwl:hasOBONamespace>
        <oboInOwl:id>GAZ:00061790</oboInOwl:id>
        <rdfs:label>Sub-Tatra Furrow</rdfs:label>
    </owl:NamedIndividual>
    


    <!-- http://purl.obolibrary.org/obo/GAZ_00061791 -->

    <owl:NamedIndividual rdf:about="http://purl.obolibrary.org/obo/GAZ_00061791">
        <obo:RO_0001025 rdf:resource="http://purl.obolibrary.org/obo/GAZ_00061750"/>
        <oboInOwl:hasOBONamespace>GAZ</oboInOwl:hasOBONamespace>
        <oboInOwl:id>GAZ:00061791</oboInOwl:id>
        <rdfs:label>Spis-Gubalowka Piedmont</rdfs:label>
    </owl:NamedIndividual>
    


    <!-- http://purl.obolibrary.org/obo/GAZ_00061792 -->

    <owl:NamedIndividual rdf:about="http://purl.obolibrary.org/obo/GAZ_00061792">
        <rdf:type rdf:resource="http://purl.obolibrary.org/obo/ENVO_00000106"/>
        <obo:RO_0001025 rdf:resource="http://purl.obolibrary.org/obo/GAZ_00061772"/>
        <obo:IAO_0000115>A Polish range of the Pieniny.</obo:IAO_0000115>
        <oboInOwl:hasOBONamespace>GAZ</oboInOwl:hasOBONamespace>
        <oboInOwl:id>GAZ:00061792</oboInOwl:id>
        <rdfs:label>Pieniny Wlasciwe</rdfs:label>
    </owl:NamedIndividual>
    


    <!-- http://purl.obolibrary.org/obo/GAZ_00061793 -->

    <owl:NamedIndividual rdf:about="http://purl.obolibrary.org/obo/GAZ_00061793">
        <rdf:type rdf:resource="http://purl.obolibrary.org/obo/ENVO_00000106"/>
        <obo:RO_0001025 rdf:resource="http://purl.obolibrary.org/obo/GAZ_00061772"/>
        <obo:IAO_0000115>A Slovak range of the Pieniny.</obo:IAO_0000115>
        <oboInOwl:hasOBONamespace>GAZ</oboInOwl:hasOBONamespace>
        <oboInOwl:id>GAZ:00061793</oboInOwl:id>
        <rdfs:label>Male Pieniny</rdfs:label>
    </owl:NamedIndividual>
    


    <!-- http://purl.obolibrary.org/obo/GAZ_00061794 -->

    <owl:NamedIndividual rdf:about="http://purl.obolibrary.org/obo/GAZ_00061794">
        <obo:RO_0001025 rdf:resource="http://purl.obolibrary.org/obo/GAZ_00061694"/>
        <obo:IAO_0000115>An extensive mountainous region of Slovakia&apos;s Spis region within the Carpathians. It is the largest mountain range in Slovakia. In the geomorphological system, the Slovenske rudohorie belongs to the Inner Western Carpathians. The mountains are bordered by Zvolen in the west, Kosice in the east, the Hron River and the Hornad River in the north, and the Juhoslovenska kotlina and Kosice Basin (Kosicka kotlina) in the south.</obo:IAO_0000115>
        <oboInOwl:hasOBONamespace>GAZ</oboInOwl:hasOBONamespace>
        <oboInOwl:id>GAZ:00061794</oboInOwl:id>
        <rdfs:label>Slovak Ore Mountains</rdfs:label>
    </owl:NamedIndividual>
    


    <!-- http://purl.obolibrary.org/obo/GAZ_00061795 -->

    <owl:NamedIndividual rdf:about="http://purl.obolibrary.org/obo/GAZ_00061795">
        <obo:RO_0001025 rdf:resource="http://purl.obolibrary.org/obo/GAZ_00061794"/>
        <oboInOwl:hasOBONamespace>GAZ</oboInOwl:hasOBONamespace>
        <oboInOwl:id>GAZ:00061795</oboInOwl:id>
        <rdfs:label>Stolica Mountains</rdfs:label>
    </owl:NamedIndividual>
    


    <!-- http://purl.obolibrary.org/obo/GAZ_00061796 -->

    <owl:NamedIndividual rdf:about="http://purl.obolibrary.org/obo/GAZ_00061796">
        <obo:RO_0001025 rdf:resource="http://purl.obolibrary.org/obo/GAZ_00061794"/>
        <oboInOwl:hasOBONamespace>GAZ</oboInOwl:hasOBONamespace>
        <oboInOwl:id>GAZ:00061796</oboInOwl:id>
        <rdfs:label>Roznava Basin</rdfs:label>
    </owl:NamedIndividual>
    


    <!-- http://purl.obolibrary.org/obo/GAZ_00061797 -->

    <owl:NamedIndividual rdf:about="http://purl.obolibrary.org/obo/GAZ_00061797">
        <obo:RO_0001025 rdf:resource="http://purl.obolibrary.org/obo/GAZ_00061794"/>
        <oboInOwl:hasOBONamespace>GAZ</oboInOwl:hasOBONamespace>
        <oboInOwl:id>GAZ:00061797</oboInOwl:id>
        <rdfs:label>Vepor Mountains</rdfs:label>
    </owl:NamedIndividual>
    


    <!-- http://purl.obolibrary.org/obo/GAZ_00061798 -->

    <owl:NamedIndividual rdf:about="http://purl.obolibrary.org/obo/GAZ_00061798">
        <obo:RO_0001025 rdf:resource="http://purl.obolibrary.org/obo/GAZ_00061794"/>
        <oboInOwl:hasOBONamespace>GAZ</oboInOwl:hasOBONamespace>
        <oboInOwl:id>GAZ:00061798</oboInOwl:id>
        <rdfs:label>Volovec Mountains</rdfs:label>
    </owl:NamedIndividual>
    


    <!-- http://purl.obolibrary.org/obo/GAZ_00061799 -->

    <owl:NamedIndividual rdf:about="http://purl.obolibrary.org/obo/GAZ_00061799">
        <obo:RO_0001025 rdf:resource="http://purl.obolibrary.org/obo/GAZ_00061794"/>
        <obo:IAO_0000115>A part (a geomorphological area) in the Slovenske rudohorie Mountains.</obo:IAO_0000115>
        <oboInOwl:hasOBONamespace>GAZ</oboInOwl:hasOBONamespace>
        <oboInOwl:id>GAZ:00061799</oboInOwl:id>
        <rdfs:label>Spis-Gemer Karst</rdfs:label>
    </owl:NamedIndividual>
    


    <!-- http://purl.obolibrary.org/obo/GAZ_00061800 -->

    <owl:NamedIndividual rdf:about="http://purl.obolibrary.org/obo/GAZ_00061800">
        <obo:RO_0001025 rdf:resource="http://purl.obolibrary.org/obo/GAZ_00061794"/>
        <obo:IAO_0000115>One of the mountain ranges of the Slovenske rudohorie Mountains in the Carpathians in southern Slovakia. It consists of a complex of huge karst plains and plateaus.</obo:IAO_0000115>
        <oboInOwl:hasOBONamespace>GAZ</oboInOwl:hasOBONamespace>
        <oboInOwl:id>GAZ:00061800</oboInOwl:id>
        <rdfs:label>Slovak Karst</rdfs:label>
    </owl:NamedIndividual>
    


    <!-- http://purl.obolibrary.org/obo/GAZ_00061801 -->

    <owl:NamedIndividual rdf:about="http://purl.obolibrary.org/obo/GAZ_00061801">
        <obo:RO_0001025 rdf:resource="http://purl.obolibrary.org/obo/GAZ_00061794"/>
        <oboInOwl:hasOBONamespace>GAZ</oboInOwl:hasOBONamespace>
        <oboInOwl:id>GAZ:00061801</oboInOwl:id>
        <rdfs:label>Cierna hora</rdfs:label>
    </owl:NamedIndividual>
    


    <!-- http://purl.obolibrary.org/obo/GAZ_00061802 -->

    <owl:NamedIndividual rdf:about="http://purl.obolibrary.org/obo/GAZ_00061802">
        <obo:RO_0001025 rdf:resource="http://purl.obolibrary.org/obo/GAZ_00061794"/>
        <oboInOwl:hasOBONamespace>GAZ</oboInOwl:hasOBONamespace>
        <oboInOwl:id>GAZ:00061802</oboInOwl:id>
        <rdfs:label>Revuca Highlands</rdfs:label>
    </owl:NamedIndividual>
    


    <!-- http://purl.obolibrary.org/obo/GAZ_00061803 -->

    <owl:NamedIndividual rdf:about="http://purl.obolibrary.org/obo/GAZ_00061803">
        <obo:RO_0001025 rdf:resource="http://purl.obolibrary.org/obo/GAZ_00061794"/>
        <oboInOwl:hasOBONamespace>GAZ</oboInOwl:hasOBONamespace>
        <oboInOwl:id>GAZ:00061803</oboInOwl:id>
        <rdfs:label>North-Borsod Karst</rdfs:label>
    </owl:NamedIndividual>
    


    <!-- http://purl.obolibrary.org/obo/GAZ_00061804 -->

    <owl:NamedIndividual rdf:about="http://purl.obolibrary.org/obo/GAZ_00061804">
        <obo:RO_0001025 rdf:resource="http://purl.obolibrary.org/obo/GAZ_00061800"/>
        <obo:IAO_0000115>A national park in the Slovak Karst (Slovensky kras) mountain range in South East Slovakia. It lies in the Gelnica, Roznava and Kosice districts in the Kosice Region. Established 2002-03-01. A World Heritage Site.</obo:IAO_0000115>
        <oboInOwl:hasOBONamespace>GAZ</oboInOwl:hasOBONamespace>
        <oboInOwl:id>GAZ:00061804</oboInOwl:id>
        <rdfs:label>Slovak Karst National Park</rdfs:label>
    </owl:NamedIndividual>
    


    <!-- http://purl.obolibrary.org/obo/GAZ_00061805 -->

    <owl:NamedIndividual rdf:about="http://purl.obolibrary.org/obo/GAZ_00061805">
        <obo:RO_0001025 rdf:resource="http://purl.obolibrary.org/obo/GAZ_00061799"/>
        <obo:IAO_0000115>A plateau-like region in central Slovakia, between Brezno, Cervena Skala (part of Sumiac), Muran and Tisovec. It lies in the Spis-Gemer Karst, in the Slovenske rudohorie Mountains (part of the Western Carpathian Mountains).</obo:IAO_0000115>
        <oboInOwl:hasOBONamespace>GAZ</oboInOwl:hasOBONamespace>
        <oboInOwl:id>GAZ:00061805</oboInOwl:id>
        <rdfs:label>Muranska planina</rdfs:label>
    </owl:NamedIndividual>
    


    <!-- http://purl.obolibrary.org/obo/GAZ_00061806 -->

    <owl:NamedIndividual rdf:about="http://purl.obolibrary.org/obo/GAZ_00061806">
        <obo:RO_0001025 rdf:resource="http://purl.obolibrary.org/obo/GAZ_00061799"/>
        <obo:IAO_0000115>A mountain range in central Slovakia. It is a part of the Spis-Gemer Karst, which in turn is a part of the Slovenske rudohorie Mountains, a major subdivision of the Western Carpathians. It is located between the towns of Spisska Nova Ves in the north and Dobsina in the south.</obo:IAO_0000115>
        <oboInOwl:hasOBONamespace>GAZ</oboInOwl:hasOBONamespace>
        <oboInOwl:id>GAZ:00061806</oboInOwl:id>
        <rdfs:label>Slovak Paradise</rdfs:label>
    </owl:NamedIndividual>
    


    <!-- http://purl.obolibrary.org/obo/GAZ_00061807 -->

    <owl:NamedIndividual rdf:about="http://purl.obolibrary.org/obo/GAZ_00061807">
        <obo:RO_0001025 rdf:resource="http://purl.obolibrary.org/obo/GAZ_00061806"/>
        <obo:IAO_0000115>A national park in Slovakia, situated in East Slovakia. The National Park protects the area of the Slovak Paradise mountain range, which is located in the north of the Slovenske rudohorie Mountains (Slovak Ore Mountains). A World Heritage Site. The National Park is situated in the Banska Bystrica Region (district of Brezno), Presov Region (district of Poprad) and Kosice Region (districts of Roznava and Spisska Nova Ves).</obo:IAO_0000115>
        <oboInOwl:hasOBONamespace>GAZ</oboInOwl:hasOBONamespace>
        <oboInOwl:id>GAZ:00061807</oboInOwl:id>
        <rdfs:label>Slovak Paradise National Park</rdfs:label>
    </owl:NamedIndividual>
    


    <!-- http://purl.obolibrary.org/obo/GAZ_00061808 -->

    <owl:NamedIndividual rdf:about="http://purl.obolibrary.org/obo/GAZ_00061808">
        <obo:RO_0001025 rdf:resource="http://purl.obolibrary.org/obo/GAZ_00061805"/>
        <obo:IAO_0000115>A national park in Slovakia. It is situated in Central Slovakia, in the districts of Brezno and Revuca, in the Banska Bystrica Region. It protects the area of Muranska planina (Muran Plateau), which is geologically part of the Slovenske rudohorie mountain range.</obo:IAO_0000115>
        <oboInOwl:hasOBONamespace>GAZ</oboInOwl:hasOBONamespace>
        <oboInOwl:id>GAZ:00061808</oboInOwl:id>
        <rdfs:label>Muranska planina National Park</rdfs:label>
    </owl:NamedIndividual>
    


    <!-- http://purl.obolibrary.org/obo/GAZ_00061809 -->

    <owl:NamedIndividual rdf:about="http://purl.obolibrary.org/obo/GAZ_00061809">
        <obo:RO_0001025 rdf:resource="http://purl.obolibrary.org/obo/GAZ_00061694"/>
        <obo:IAO_0000115>A part of the Inner Western Carpathians, a subprovince of the Carpathians. Most of the area lies in Slovakia with small parts reaching into Austria and Poland.</obo:IAO_0000115>
        <oboInOwl:hasOBONamespace>GAZ</oboInOwl:hasOBONamespace>
        <oboInOwl:id>GAZ:00061809</oboInOwl:id>
        <rdfs:label>Fatra-Tatra Area</rdfs:label>
    </owl:NamedIndividual>
    


    <!-- http://purl.obolibrary.org/obo/GAZ_00061810 -->

    <owl:NamedIndividual rdf:about="http://purl.obolibrary.org/obo/GAZ_00061810">
        <obo:RO_0001025 rdf:resource="http://purl.obolibrary.org/obo/GAZ_00005403"/>
        <obo:IAO_0000115>The region of the Little Carpathians rom Bratislava to Bukova.</obo:IAO_0000115>
        <oboInOwl:hasOBONamespace>GAZ</oboInOwl:hasOBONamespace>
        <oboInOwl:id>GAZ:00061810</oboInOwl:id>
        <rdfs:label>Pezinok Carpathians</rdfs:label>
    </owl:NamedIndividual>
    


    <!-- http://purl.obolibrary.org/obo/GAZ_00061811 -->

    <owl:NamedIndividual rdf:about="http://purl.obolibrary.org/obo/GAZ_00061811">
        <obo:RO_0001025 rdf:resource="http://purl.obolibrary.org/obo/GAZ_00005403"/>
        <obo:IAO_0000115>The region of the Little Carpathians in Bratislava.</obo:IAO_0000115>
        <oboInOwl:hasOBONamespace>GAZ</oboInOwl:hasOBONamespace>
        <oboInOwl:id>GAZ:00061811</oboInOwl:id>
        <rdfs:label>Devin Carpathians</rdfs:label>
    </owl:NamedIndividual>
    


    <!-- http://purl.obolibrary.org/obo/GAZ_00061812 -->

    <owl:NamedIndividual rdf:about="http://purl.obolibrary.org/obo/GAZ_00061812">
        <obo:RO_0001025 rdf:resource="http://purl.obolibrary.org/obo/GAZ_00005403"/>
        <obo:IAO_0000115>The region of the Little Carpathians from Prasnik to Nove Mesto nad Vahom.</obo:IAO_0000115>
        <oboInOwl:hasOBONamespace>GAZ</oboInOwl:hasOBONamespace>
        <oboInOwl:id>GAZ:00061812</oboInOwl:id>
        <rdfs:label>Cachtice Carpathians</rdfs:label>
    </owl:NamedIndividual>
    


    <!-- http://purl.obolibrary.org/obo/GAZ_00061813 -->

    <owl:NamedIndividual rdf:about="http://purl.obolibrary.org/obo/GAZ_00061813">
        <obo:RO_0001025 rdf:resource="http://purl.obolibrary.org/obo/GAZ_00005403"/>
        <obo:IAO_0000115>The region of the Little Carpathians from Bukova to Prasnik.</obo:IAO_0000115>
        <oboInOwl:hasOBONamespace>GAZ</oboInOwl:hasOBONamespace>
        <oboInOwl:id>GAZ:00061813</oboInOwl:id>
        <rdfs:label>Brezova Carpathians</rdfs:label>
    </owl:NamedIndividual>
    


    <!-- http://purl.obolibrary.org/obo/GAZ_00061814 -->

    <owl:NamedIndividual rdf:about="http://purl.obolibrary.org/obo/GAZ_00061814">
        <obo:RO_0001025 rdf:resource="http://purl.obolibrary.org/obo/GAZ_00061809"/>
        <obo:IAO_0000115>A 48 km long and 15-25 km wide mountain range. It is situated from the city of Hlohovec, raising from the Danubian Hills, and slowly raising further north until nearly to the city of Trencin where it borders the Strazov Mountains, where is also the highest hill of the entire mountain range, Inovec (1042 m). The mountain range separates basins of the Vah and Nitra rivers.</obo:IAO_0000115>
        <oboInOwl:hasOBONamespace>GAZ</oboInOwl:hasOBONamespace>
        <oboInOwl:id>GAZ:00061814</oboInOwl:id>
        <rdfs:label>Povassky Inovec</rdfs:label>
    </owl:NamedIndividual>
    


    <!-- http://purl.obolibrary.org/obo/GAZ_00061815 -->

    <owl:NamedIndividual rdf:about="http://purl.obolibrary.org/obo/GAZ_00061815">
        <obo:RO_0001025 rdf:resource="http://purl.obolibrary.org/obo/GAZ_00061809"/>
        <oboInOwl:hasOBONamespace>GAZ</oboInOwl:hasOBONamespace>
        <oboInOwl:id>GAZ:00061815</oboInOwl:id>
        <rdfs:label>Tribec Mountains</rdfs:label>
    </owl:NamedIndividual>
    


    <!-- http://purl.obolibrary.org/obo/GAZ_00061816 -->

    <owl:NamedIndividual rdf:about="http://purl.obolibrary.org/obo/GAZ_00061816">
        <obo:RO_0001025 rdf:resource="http://purl.obolibrary.org/obo/GAZ_00061809"/>
        <obo:IAO_0000115>A mountain range in northwestern Slovakia, being part of Inner Western Carpathians, and of the Fatra-Tatra Area. They are situated between the towns of Trencin, Povazska Bystrica, Rajec, Prievidza and Banovce nad Bebravou, bordering White Carpathians and the Vah river in the northwest and west, Javorniky in the north, Mala Fatra in the east, Vtacnik and Nitra river in the south and Vah Inovec in the southwest.</obo:IAO_0000115>
        <oboInOwl:hasOBONamespace>GAZ</oboInOwl:hasOBONamespace>
        <oboInOwl:id>GAZ:00061816</oboInOwl:id>
        <rdfs:label>Strazov Mountains</rdfs:label>
    </owl:NamedIndividual>
    


    <!-- http://purl.obolibrary.org/obo/GAZ_00061817 -->

    <owl:NamedIndividual rdf:about="http://purl.obolibrary.org/obo/GAZ_00061817">
        <obo:RO_0001025 rdf:resource="http://purl.obolibrary.org/obo/GAZ_00061809"/>
        <oboInOwl:hasOBONamespace>GAZ</oboInOwl:hasOBONamespace>
        <oboInOwl:id>GAZ:00061817</oboInOwl:id>
        <rdfs:label>Ziar</rdfs:label>
    </owl:NamedIndividual>
    


    <!-- http://purl.obolibrary.org/obo/GAZ_00061818 -->

    <owl:NamedIndividual rdf:about="http://purl.obolibrary.org/obo/GAZ_00061818">
        <obo:RO_0001025 rdf:resource="http://purl.obolibrary.org/obo/GAZ_00061809"/>
        <obo:IAO_0000115>A mountain range in the Western Carpathians in the north-west of Central Slovakia. In the geomorphological system, it is a part of the Fatra-Tatra Area. It is situated approximately between the cities of Nitrianske Pravno, Strecno, Martin and Zszriva. Turcianska kotlina (Turiec Basin) and the Oravska vrchovina Mountains are situated to the west of the range, and Zilinska kotlina (Zilina Basin) and the Kysucka vrchovina Mountains are located to the east. Mala Fatra consists of two subdivisions separated by the Vah river near Strecno.</obo:IAO_0000115>
        <oboInOwl:hasOBONamespace>GAZ</oboInOwl:hasOBONamespace>
        <oboInOwl:id>GAZ:00061818</oboInOwl:id>
        <rdfs:label>Mala Fatra</rdfs:label>
    </owl:NamedIndividual>
    


    <!-- http://purl.obolibrary.org/obo/GAZ_00061819 -->

    <owl:NamedIndividual rdf:about="http://purl.obolibrary.org/obo/GAZ_00061819">
        <obo:RO_0001025 rdf:resource="http://purl.obolibrary.org/obo/GAZ_00061809"/>
        <oboInOwl:hasOBONamespace>GAZ</oboInOwl:hasOBONamespace>
        <oboInOwl:id>GAZ:00061819</oboInOwl:id>
        <rdfs:label>Su&apos;lov Mountains</rdfs:label>
    </owl:NamedIndividual>
    


    <!-- http://purl.obolibrary.org/obo/GAZ_00061820 -->

    <owl:NamedIndividual rdf:about="http://purl.obolibrary.org/obo/GAZ_00061820">
        <obo:RO_0001025 rdf:resource="http://purl.obolibrary.org/obo/GAZ_00061818"/>
        <oboInOwl:hasOBONamespace>GAZ</oboInOwl:hasOBONamespace>
        <oboInOwl:id>GAZ:00061820</oboInOwl:id>
        <rdfs:label>Lucanska Mala Fatra</rdfs:label>
    </owl:NamedIndividual>
    


    <!-- http://purl.obolibrary.org/obo/GAZ_00061821 -->

    <owl:NamedIndividual rdf:about="http://purl.obolibrary.org/obo/GAZ_00061821">
        <obo:RO_0001025 rdf:resource="http://purl.obolibrary.org/obo/GAZ_00061818"/>
        <oboInOwl:hasOBONamespace>GAZ</oboInOwl:hasOBONamespace>
        <oboInOwl:id>GAZ:00061821</oboInOwl:id>
        <rdfs:label>Krivanska Mala Fatra</rdfs:label>
    </owl:NamedIndividual>
    


    <!-- http://purl.obolibrary.org/obo/GAZ_00061822 -->

    <owl:NamedIndividual rdf:about="http://purl.obolibrary.org/obo/GAZ_00061822">
        <obo:RO_0001025 rdf:resource="http://purl.obolibrary.org/obo/GAZ_00061809"/>
        <obo:IAO_0000115>A mountain range in the Western Carpathians in Slovakia. In the geomorphological system, it is a part of the Fatra-Tatra Area. It is situated approximately among the towns of Ruzomberok, Harmanec, Turcianske Teplice and Martin. The Turiec Basin and the Lesser Fatra mountains are situated to the north west of the range and the Low Tatras mountains are in the east. It can be divided into 7 parts.</obo:IAO_0000115>
        <oboInOwl:hasOBONamespace>GAZ</oboInOwl:hasOBONamespace>
        <oboInOwl:id>GAZ:00061822</oboInOwl:id>
        <rdfs:label>Vel&apos;ka Fatra</rdfs:label>
    </owl:NamedIndividual>
    


    <!-- http://purl.obolibrary.org/obo/GAZ_00061823 -->

    <owl:NamedIndividual rdf:about="http://purl.obolibrary.org/obo/GAZ_00061823">
        <obo:RO_0001025 rdf:resource="http://purl.obolibrary.org/obo/GAZ_00061809"/>
        <obo:IAO_0000115>A small mountain range in Central Slovakia, near the town of Banska Bystrica. It is a part of the Low Tatra, which is part of the Fatra-Tatra Area and the Inner Western Carpathians. It borders the Ve&apos;ka Fatra Mountains in the north west and north, Low Tatra in the east, Zvolen Basin in the south and the Kremnica Mountains in the west.</obo:IAO_0000115>
        <oboInOwl:hasOBONamespace>GAZ</oboInOwl:hasOBONamespace>
        <oboInOwl:id>GAZ:00061823</oboInOwl:id>
        <rdfs:label>Stare Hory Mountains</rdfs:label>
    </owl:NamedIndividual>
    


    <!-- http://purl.obolibrary.org/obo/GAZ_00061824 -->

    <owl:NamedIndividual rdf:about="http://purl.obolibrary.org/obo/GAZ_00061824">
        <obo:RO_0001025 rdf:resource="http://purl.obolibrary.org/obo/GAZ_00061822"/>
        <oboInOwl:hasOBONamespace>GAZ</oboInOwl:hasOBONamespace>
        <oboInOwl:id>GAZ:00061824</oboInOwl:id>
        <rdfs:label>Revucke podolie</rdfs:label>
    </owl:NamedIndividual>
    


    <!-- http://purl.obolibrary.org/obo/GAZ_00061825 -->

    <owl:NamedIndividual rdf:about="http://purl.obolibrary.org/obo/GAZ_00061825">
        <obo:RO_0001025 rdf:resource="http://purl.obolibrary.org/obo/GAZ_00061822"/>
        <oboInOwl:hasOBONamespace>GAZ</oboInOwl:hasOBONamespace>
        <oboInOwl:id>GAZ:00061825</oboInOwl:id>
        <rdfs:label>Zvolen</rdfs:label>
    </owl:NamedIndividual>
    


    <!-- http://purl.obolibrary.org/obo/GAZ_00061826 -->

    <owl:NamedIndividual rdf:about="http://purl.obolibrary.org/obo/GAZ_00061826">
        <obo:RO_0001025 rdf:resource="http://purl.obolibrary.org/obo/GAZ_00061822"/>
        <oboInOwl:hasOBONamespace>GAZ</oboInOwl:hasOBONamespace>
        <oboInOwl:id>GAZ:00061826</oboInOwl:id>
        <rdfs:label>Bralna Fatra</rdfs:label>
    </owl:NamedIndividual>
    


    <!-- http://purl.obolibrary.org/obo/GAZ_00061827 -->

    <owl:NamedIndividual rdf:about="http://purl.obolibrary.org/obo/GAZ_00061827">
        <obo:RO_0001025 rdf:resource="http://purl.obolibrary.org/obo/GAZ_00061822"/>
        <oboInOwl:hasOBONamespace>GAZ</oboInOwl:hasOBONamespace>
        <oboInOwl:id>GAZ:00061827</oboInOwl:id>
        <rdfs:label>Sipska Fatra</rdfs:label>
    </owl:NamedIndividual>
    


    <!-- http://purl.obolibrary.org/obo/GAZ_00061828 -->

    <owl:NamedIndividual rdf:about="http://purl.obolibrary.org/obo/GAZ_00061828">
        <obo:RO_0001025 rdf:resource="http://purl.obolibrary.org/obo/GAZ_00061822"/>
        <oboInOwl:hasOBONamespace>GAZ</oboInOwl:hasOBONamespace>
        <oboInOwl:id>GAZ:00061828</oboInOwl:id>
        <rdfs:label>Siprun</rdfs:label>
    </owl:NamedIndividual>
    


    <!-- http://purl.obolibrary.org/obo/GAZ_00061829 -->

    <owl:NamedIndividual rdf:about="http://purl.obolibrary.org/obo/GAZ_00061829">
        <obo:RO_0001025 rdf:resource="http://purl.obolibrary.org/obo/GAZ_00061822"/>
        <oboInOwl:hasOBONamespace>GAZ</oboInOwl:hasOBONamespace>
        <oboInOwl:id>GAZ:00061829</oboInOwl:id>
        <rdfs:label>Hol&apos;na Fatra</rdfs:label>
    </owl:NamedIndividual>
    


    <!-- http://purl.obolibrary.org/obo/GAZ_00061830 -->

    <owl:NamedIndividual rdf:about="http://purl.obolibrary.org/obo/GAZ_00061830">
        <obo:RO_0001025 rdf:resource="http://purl.obolibrary.org/obo/GAZ_00061822"/>
        <oboInOwl:hasOBONamespace>GAZ</oboInOwl:hasOBONamespace>
        <oboInOwl:id>GAZ:00061830</oboInOwl:id>
        <rdfs:label>Lysec</rdfs:label>
    </owl:NamedIndividual>
    


    <!-- http://purl.obolibrary.org/obo/GAZ_00061831 -->

    <owl:NamedIndividual rdf:about="http://purl.obolibrary.org/obo/GAZ_00061831">
        <obo:RO_0001025 rdf:resource="http://purl.obolibrary.org/obo/GAZ_00061809"/>
        <oboInOwl:hasOBONamespace>GAZ</oboInOwl:hasOBONamespace>
        <oboInOwl:id>GAZ:00061831</oboInOwl:id>
        <rdfs:label>Choc Mountains</rdfs:label>
    </owl:NamedIndividual>
    


    <!-- http://purl.obolibrary.org/obo/GAZ_00061832 -->

    <owl:NamedIndividual rdf:about="http://purl.obolibrary.org/obo/GAZ_00061832">
        <obo:RO_0001025 rdf:resource="http://purl.obolibrary.org/obo/GAZ_00481063"/>
        <obo:IAO_0000115>A lake in the High Tatras.</obo:IAO_0000115>
        <oboInOwl:hasOBONamespace>GAZ</oboInOwl:hasOBONamespace>
        <oboInOwl:id>GAZ:00061832</oboInOwl:id>
        <rdfs:label>Wielki Staw Polski</rdfs:label>
    </owl:NamedIndividual>
    


    <!-- http://purl.obolibrary.org/obo/GAZ_00061833 -->

    <owl:NamedIndividual rdf:about="http://purl.obolibrary.org/obo/GAZ_00061833">
        <obo:IAO_0000115>A lake located in the Lesser Poland Voivodeship. It is situated in the Rybi Potok Valley, at the base of the Mieguszowiecki Summits, and deep within the Tatra National Park.</obo:IAO_0000115>
        <oboInOwl:hasOBONamespace>GAZ</oboInOwl:hasOBONamespace>
        <oboInOwl:id>GAZ:00061833</oboInOwl:id>
        <rdfs:label>Morskie Oko</rdfs:label>
    </owl:NamedIndividual>
    


    <!-- http://purl.obolibrary.org/obo/GAZ_00061835 -->

    <owl:NamedIndividual rdf:about="http://purl.obolibrary.org/obo/GAZ_00061835">
        <obo:IAO_0000115>A lake in the High Tatras.</obo:IAO_0000115>
        <oboInOwl:hasOBONamespace>GAZ</oboInOwl:hasOBONamespace>
        <oboInOwl:id>GAZ:00061835</oboInOwl:id>
        <rdfs:label>Ve&apos;ke Hincovo pleso</rdfs:label>
    </owl:NamedIndividual>
    


    <!-- http://purl.obolibrary.org/obo/GAZ_00061839 -->

    <owl:NamedIndividual rdf:about="http://purl.obolibrary.org/obo/GAZ_00061839">
        <obo:IAO_0000115>A lake in the High Tatras.</obo:IAO_0000115>
        <oboInOwl:hasOBONamespace>GAZ</oboInOwl:hasOBONamespace>
        <oboInOwl:id>GAZ:00061839</oboInOwl:id>
        <rdfs:label>L&apos;adove pleso</rdfs:label>
    </owl:NamedIndividual>
    


    <!-- http://purl.obolibrary.org/obo/GAZ_00061844 -->

    <owl:NamedIndividual rdf:about="http://purl.obolibrary.org/obo/GAZ_00061844">
        <obo:IAO_0000115>A lake in the High Tatras.</obo:IAO_0000115>
        <oboInOwl:hasOBONamespace>GAZ</oboInOwl:hasOBONamespace>
        <oboInOwl:id>GAZ:00061844</oboInOwl:id>
        <rdfs:label>Vel&apos;ke Spisske pleso</rdfs:label>
    </owl:NamedIndividual>
    


    <!-- http://purl.obolibrary.org/obo/GAZ_00061846 -->

    <owl:NamedIndividual rdf:about="http://purl.obolibrary.org/obo/GAZ_00061846">
        <obo:RO_0001025 rdf:resource="http://purl.obolibrary.org/obo/GAZ_00481031"/>
        <obo:IAO_0000115>A lake in the High Tatras.</obo:IAO_0000115>
        <oboInOwl:hasOBONamespace>GAZ</oboInOwl:hasOBONamespace>
        <oboInOwl:id>GAZ:00061846</oboInOwl:id>
        <rdfs:label>Czarny Staw Gasienic</rdfs:label>
    </owl:NamedIndividual>
    


    <!-- http://purl.obolibrary.org/obo/GAZ_00061848 -->

    <owl:NamedIndividual rdf:about="http://purl.obolibrary.org/obo/GAZ_00061848">
        <obo:RO_0001025 rdf:resource="http://purl.obolibrary.org/obo/GAZ_00056820"/>
        <obo:IAO_0000115>A national park located in the southern part of Poland, by the borders with Slovakia. It was created in 1954.</obo:IAO_0000115>
        <oboInOwl:hasOBONamespace>GAZ</oboInOwl:hasOBONamespace>
        <oboInOwl:id>GAZ:00061848</oboInOwl:id>
        <rdfs:label>Tatrzanski Park Narodowy</rdfs:label>
    </owl:NamedIndividual>
    


    <!-- http://purl.obolibrary.org/obo/GAZ_00061849 -->

    <owl:NamedIndividual rdf:about="http://purl.obolibrary.org/obo/GAZ_00061849">
        <obo:RO_0001025 rdf:resource="http://purl.obolibrary.org/obo/GAZ_00007973"/>
        <obo:IAO_0000115>A national park in Central Slovakia, between the Vah River and the Hron River valleys. The park and its buffer zone cover the whole Low Tatras mountain range. It is divided between the Banska Bystrica Region (Banska Bystrica and Brezno districts), Zilina Region (Ruzomberok and Liptovsky Mikulas districts) and Presov Region (Poprad District). Established in 1978.</obo:IAO_0000115>
        <oboInOwl:hasOBONamespace>GAZ</oboInOwl:hasOBONamespace>
        <oboInOwl:id>GAZ:00061849</oboInOwl:id>
        <rdfs:label>Low Tatras National Park</rdfs:label>
    </owl:NamedIndividual>
    


    <!-- http://purl.obolibrary.org/obo/GAZ_00061850 -->

    <owl:NamedIndividual rdf:about="http://purl.obolibrary.org/obo/GAZ_00061850">
        <obo:RO_0001025 rdf:resource="http://purl.obolibrary.org/obo/GAZ_00061809"/>
        <oboInOwl:hasOBONamespace>GAZ</oboInOwl:hasOBONamespace>
        <oboInOwl:id>GAZ:00061850</oboInOwl:id>
        <rdfs:label>Zilina Basin</rdfs:label>
    </owl:NamedIndividual>
    


    <!-- http://purl.obolibrary.org/obo/GAZ_00061851 -->

    <owl:NamedIndividual rdf:about="http://purl.obolibrary.org/obo/GAZ_00061851">
        <obo:RO_0001025 rdf:resource="http://purl.obolibrary.org/obo/GAZ_00061809"/>
        <oboInOwl:hasOBONamespace>GAZ</oboInOwl:hasOBONamespace>
        <oboInOwl:id>GAZ:00061851</oboInOwl:id>
        <rdfs:label>Turiec Basin</rdfs:label>
    </owl:NamedIndividual>
    


    <!-- http://purl.obolibrary.org/obo/GAZ_00061852 -->

    <owl:NamedIndividual rdf:about="http://purl.obolibrary.org/obo/GAZ_00061852">
        <obo:RO_0001025 rdf:resource="http://purl.obolibrary.org/obo/GAZ_00061809"/>
        <oboInOwl:hasOBONamespace>GAZ</oboInOwl:hasOBONamespace>
        <oboInOwl:id>GAZ:00061852</oboInOwl:id>
        <rdfs:label>Hornad Basin</rdfs:label>
    </owl:NamedIndividual>
    


    <!-- http://purl.obolibrary.org/obo/GAZ_00061853 -->

    <owl:NamedIndividual rdf:about="http://purl.obolibrary.org/obo/GAZ_00061853">
        <rdf:type rdf:resource="http://purl.obolibrary.org/obo/ENVO_00000104"/>
        <obo:RO_0001025 rdf:resource="http://purl.obolibrary.org/obo/GAZ_00061809"/>
        <obo:IAO_0000115>A basin in Slovakia, part of the Fatra-Tatra Area, which belongs to the Inner Western Carpathians. It is located in northern Slovakia. It is oriented in the east-west axis around 80 km long with around 10 km width in north-south direction. It borders: N, Tatras; NE, Spisska Magura; E, Levoca Hills; S, Low Tatras; SWm Greater Fatra; NW, Chocske vrchy. The basin is divided into three sub-divisions. The border between these is also the drainage divide; the Vah River drains western part of the area and flows into Danube, which flows into the Black Sea, and the Poprad River drains the eastern part and flows through Dunajec into Vistula, which flows into the Baltic Sea.</obo:IAO_0000115>
        <oboInOwl:hasOBONamespace>GAZ</oboInOwl:hasOBONamespace>
        <oboInOwl:id>GAZ:00061853</oboInOwl:id>
        <rdfs:label>Podtatranska kotlina</rdfs:label>
    </owl:NamedIndividual>
    


    <!-- http://purl.obolibrary.org/obo/GAZ_00061854 -->

    <owl:NamedIndividual rdf:about="http://purl.obolibrary.org/obo/GAZ_00061854">
        <obo:RO_0001025 rdf:resource="http://purl.obolibrary.org/obo/GAZ_00061809"/>
        <obo:IAO_0000115>A mountainous area in Slovakia, part of the Carpathian Mountains. The Kozie chrbty is located between the High Tatras and the Low Tatras, south and west of Poprad. They are drained by the river Vah to the west, and the rivers Hornad and Poprad to the east.</obo:IAO_0000115>
        <oboInOwl:hasOBONamespace>GAZ</oboInOwl:hasOBONamespace>
        <oboInOwl:id>GAZ:00061854</oboInOwl:id>
        <rdfs:label>Kozie chrbty</rdfs:label>
    </owl:NamedIndividual>
    


    <!-- http://purl.obolibrary.org/obo/GAZ_00061855 -->

    <owl:NamedIndividual rdf:about="http://purl.obolibrary.org/obo/GAZ_00061855">
        <obo:RO_0001025 rdf:resource="http://purl.obolibrary.org/obo/GAZ_00061809"/>
        <oboInOwl:hasOBONamespace>GAZ</oboInOwl:hasOBONamespace>
        <oboInOwl:id>GAZ:00061855</oboInOwl:id>
        <rdfs:label>Horehronske podolie</rdfs:label>
    </owl:NamedIndividual>
    


    <!-- http://purl.obolibrary.org/obo/GAZ_00061856 -->

    <owl:NamedIndividual rdf:about="http://purl.obolibrary.org/obo/GAZ_00061856">
        <obo:RO_0001025 rdf:resource="http://purl.obolibrary.org/obo/GAZ_00061809"/>
        <obo:IAO_0000115>A mountain range in eastern Slovakia, between the Spis and Saris regions. It is 16 km long mountain range in the north-south direction, belonging to the Outer Western Carpathians.</obo:IAO_0000115>
        <oboInOwl:hasOBONamespace>GAZ</oboInOwl:hasOBONamespace>
        <oboInOwl:id>GAZ:00061856</oboInOwl:id>
        <rdfs:label>Branisko</rdfs:label>
    </owl:NamedIndividual>
    


    <!-- http://purl.obolibrary.org/obo/GAZ_00061857 -->

    <owl:NamedIndividual rdf:about="http://purl.obolibrary.org/obo/GAZ_00061857">
        <obo:RO_0001025 rdf:resource="http://purl.obolibrary.org/obo/GAZ_00061809"/>
        <oboInOwl:hasOBONamespace>GAZ</oboInOwl:hasOBONamespace>
        <oboInOwl:id>GAZ:00061857</oboInOwl:id>
        <rdfs:label>Upper Nitra Basin</rdfs:label>
    </owl:NamedIndividual>
    


    <!-- http://purl.obolibrary.org/obo/GAZ_00061858 -->

    <owl:NamedIndividual rdf:about="http://purl.obolibrary.org/obo/GAZ_00061858">
        <obo:RO_0001025 rdf:resource="http://purl.obolibrary.org/obo/GAZ_00061809"/>
        <oboInOwl:hasOBONamespace>GAZ</oboInOwl:hasOBONamespace>
        <oboInOwl:id>GAZ:00061858</oboInOwl:id>
        <rdfs:label>Hainburg Mountains</rdfs:label>
    </owl:NamedIndividual>
    


    <!-- http://purl.obolibrary.org/obo/GAZ_00061859 -->

    <owl:NamedIndividual rdf:about="http://purl.obolibrary.org/obo/GAZ_00061859">
        <obo:RO_0001025 rdf:resource="http://purl.obolibrary.org/obo/GAZ_00061853"/>
        <oboInOwl:hasOBONamespace>GAZ</oboInOwl:hasOBONamespace>
        <oboInOwl:id>GAZ:00061859</oboInOwl:id>
        <rdfs:label>Liptovska kotlina</rdfs:label>
    </owl:NamedIndividual>
    


    <!-- http://purl.obolibrary.org/obo/GAZ_00061860 -->

    <owl:NamedIndividual rdf:about="http://purl.obolibrary.org/obo/GAZ_00061860">
        <obo:RO_0001025 rdf:resource="http://purl.obolibrary.org/obo/GAZ_00061853"/>
        <oboInOwl:hasOBONamespace>GAZ</oboInOwl:hasOBONamespace>
        <oboInOwl:id>GAZ:00061860</oboInOwl:id>
        <rdfs:label>Tatranske predhorie</rdfs:label>
    </owl:NamedIndividual>
    


    <!-- http://purl.obolibrary.org/obo/GAZ_00061861 -->

    <owl:NamedIndividual rdf:about="http://purl.obolibrary.org/obo/GAZ_00061861">
        <obo:RO_0001025 rdf:resource="http://purl.obolibrary.org/obo/GAZ_00061853"/>
        <oboInOwl:hasOBONamespace>GAZ</oboInOwl:hasOBONamespace>
        <oboInOwl:id>GAZ:00061861</oboInOwl:id>
        <rdfs:label>Popradska kotlina</rdfs:label>
    </owl:NamedIndividual>
    


    <!-- http://purl.obolibrary.org/obo/GAZ_00061862 -->

    <owl:NamedIndividual rdf:about="http://purl.obolibrary.org/obo/GAZ_00061862">
        <obo:RO_0001025 rdf:resource="http://purl.obolibrary.org/obo/GAZ_00061694"/>
        <obo:IAO_0000115>A group of mountain ranges in southern central Slovakia. Approximately in the center of the mountains lies the city of Zvolen. Slovenske stredohorie is a part of the Inner Western Carpathians. They are bordered by the Fatra-Tatra Area in the northwest and north, Slovenske rudohorie (Slovak Ore Mountains) in the east, Juhoslovenska kotlina basin in the south and by the Pannonian Plain in the southwest.</obo:IAO_0000115>
        <oboInOwl:hasOBONamespace>GAZ</oboInOwl:hasOBONamespace>
        <oboInOwl:id>GAZ:00061862</oboInOwl:id>
        <rdfs:label>Slovenske stredohorie</rdfs:label>
    </owl:NamedIndividual>
    


    <!-- http://purl.obolibrary.org/obo/GAZ_00061863 -->

    <owl:NamedIndividual rdf:about="http://purl.obolibrary.org/obo/GAZ_00061863">
        <obo:RO_0001025 rdf:resource="http://purl.obolibrary.org/obo/GAZ_00061862"/>
        <oboInOwl:hasOBONamespace>GAZ</oboInOwl:hasOBONamespace>
        <oboInOwl:id>GAZ:00061863</oboInOwl:id>
        <rdfs:label>Hron Inovec</rdfs:label>
    </owl:NamedIndividual>
    


    <!-- http://purl.obolibrary.org/obo/GAZ_00061864 -->

    <owl:NamedIndividual rdf:about="http://purl.obolibrary.org/obo/GAZ_00061864">
        <obo:RO_0001025 rdf:resource="http://purl.obolibrary.org/obo/GAZ_00061862"/>
        <oboInOwl:hasOBONamespace>GAZ</oboInOwl:hasOBONamespace>
        <oboInOwl:id>GAZ:00061864</oboInOwl:id>
        <rdfs:label>Ostrozky</rdfs:label>
    </owl:NamedIndividual>
    


    <!-- http://purl.obolibrary.org/obo/GAZ_00061865 -->

    <owl:NamedIndividual rdf:about="http://purl.obolibrary.org/obo/GAZ_00061865">
        <obo:RO_0001025 rdf:resource="http://purl.obolibrary.org/obo/GAZ_00061862"/>
        <obo:IAO_0000115>A mountain range in central Slovakia, which is part of the Slovenske stredohorie Mountains and part of the Inner Western Carpathians. It is bordered in the west, north and northeast by the upper Nitra basin, Strazov Mountains and Ziar, in the east by the Kremnica Mountains and Ziar basin, and in the south by Tribec and the Stiavnica Mountains.</obo:IAO_0000115>
        <oboInOwl:hasOBONamespace>GAZ</oboInOwl:hasOBONamespace>
        <oboInOwl:id>GAZ:00061865</oboInOwl:id>
        <rdfs:label>Vtacnik Mountains</rdfs:label>
    </owl:NamedIndividual>
    


    <!-- http://purl.obolibrary.org/obo/GAZ_00061866 -->

    <owl:NamedIndividual rdf:about="http://purl.obolibrary.org/obo/GAZ_00061866">
        <obo:RO_0001025 rdf:resource="http://purl.obolibrary.org/obo/GAZ_00061862"/>
        <oboInOwl:hasOBONamespace>GAZ</oboInOwl:hasOBONamespace>
        <oboInOwl:id>GAZ:00061866</oboInOwl:id>
        <rdfs:label>Zvolen Basin</rdfs:label>
    </owl:NamedIndividual>
    


    <!-- http://purl.obolibrary.org/obo/GAZ_00061867 -->

    <owl:NamedIndividual rdf:about="http://purl.obolibrary.org/obo/GAZ_00061867">
        <obo:RO_0001025 rdf:resource="http://purl.obolibrary.org/obo/GAZ_00061862"/>
        <oboInOwl:hasOBONamespace>GAZ</oboInOwl:hasOBONamespace>
        <oboInOwl:id>GAZ:00061867</oboInOwl:id>
        <rdfs:label>Javorie</rdfs:label>
    </owl:NamedIndividual>
    


    <!-- http://purl.obolibrary.org/obo/GAZ_00061868 -->

    <owl:NamedIndividual rdf:about="http://purl.obolibrary.org/obo/GAZ_00061868">
        <obo:RO_0001025 rdf:resource="http://purl.obolibrary.org/obo/GAZ_00061862"/>
        <obo:IAO_0000115>A volcanic mountain range in southern central Slovakia. They are part of Inner Western Carpathians and the Slovenske stredohorie Mountains. The area is protected by Stiavnica Mountains Protected Landscape Area. They are bordered by the Kremnica Mountains (Kremnicke vrchy) in the north, Pliesovce and Krupina basins (Krupinska kotlina) in the east, Danubian Hills (Podunajska pahorkatina) in the south and Pohronsky Inovec, Vtacnik and Ziar Basin (Ziarska kotlina) in the west.</obo:IAO_0000115>
        <oboInOwl:hasOBONamespace>GAZ</oboInOwl:hasOBONamespace>
        <oboInOwl:id>GAZ:00061868</oboInOwl:id>
        <rdfs:label>Stiavnica Mountains</rdfs:label>
    </owl:NamedIndividual>
    


    <!-- http://purl.obolibrary.org/obo/GAZ_00061869 -->

    <owl:NamedIndividual rdf:about="http://purl.obolibrary.org/obo/GAZ_00061869">
        <obo:RO_0001025 rdf:resource="http://purl.obolibrary.org/obo/GAZ_00061862"/>
        <oboInOwl:hasOBONamespace>GAZ</oboInOwl:hasOBONamespace>
        <oboInOwl:id>GAZ:00061869</oboInOwl:id>
        <rdfs:label>Pliesovce Basin</rdfs:label>
    </owl:NamedIndividual>
    


    <!-- http://purl.obolibrary.org/obo/GAZ_00061870 -->

    <owl:NamedIndividual rdf:about="http://purl.obolibrary.org/obo/GAZ_00061870">
        <obo:RO_0001025 rdf:resource="http://purl.obolibrary.org/obo/GAZ_00061862"/>
        <oboInOwl:hasOBONamespace>GAZ</oboInOwl:hasOBONamespace>
        <oboInOwl:id>GAZ:00061870</oboInOwl:id>
        <rdfs:label>Krupina Plain</rdfs:label>
    </owl:NamedIndividual>
    


    <!-- http://purl.obolibrary.org/obo/GAZ_00061871 -->

    <owl:NamedIndividual rdf:about="http://purl.obolibrary.org/obo/GAZ_00061871">
        <obo:RO_0001025 rdf:resource="http://purl.obolibrary.org/obo/GAZ_00061862"/>
        <oboInOwl:hasOBONamespace>GAZ</oboInOwl:hasOBONamespace>
        <oboInOwl:id>GAZ:00061871</oboInOwl:id>
        <rdfs:label>Ziar Basin</rdfs:label>
    </owl:NamedIndividual>
    


    <!-- http://purl.obolibrary.org/obo/GAZ_00061872 -->

    <owl:NamedIndividual rdf:about="http://purl.obolibrary.org/obo/GAZ_00061872">
        <obo:RO_0001025 rdf:resource="http://purl.obolibrary.org/obo/GAZ_00061862"/>
        <obo:IAO_0000115>Part of the Slovenske stredohorie.</obo:IAO_0000115>
        <oboInOwl:hasOBONamespace>GAZ</oboInOwl:hasOBONamespace>
        <oboInOwl:id>GAZ:00061872</oboInOwl:id>
        <rdfs:label>Polana Mountains</rdfs:label>
    </owl:NamedIndividual>
    


    <!-- http://purl.obolibrary.org/obo/GAZ_00061873 -->

    <owl:NamedIndividual rdf:about="http://purl.obolibrary.org/obo/GAZ_00061873">
        <obo:RO_0001025 rdf:resource="http://purl.obolibrary.org/obo/GAZ_00061862"/>
        <obo:IAO_0000115>A volcanic mountain range in central Slovakia. They are part of the Western Carpathians and the Slovenske stredohorie Mts. The mountain range is situated east of the town of Kremnica, which gave it its name. It is bordered by Ve&apos;ka Fatra and Turiec Basin (Turcianska kotlina) in the north, Zvolen Basin (Zvolenska kotlina) in the east, Ziar Basin (Ziarska kotlina) and Stiavnica Mountains (Stiavnicke vrchy) in the south, and Vtacnik in the west.</obo:IAO_0000115>
        <oboInOwl:hasOBONamespace>GAZ</oboInOwl:hasOBONamespace>
        <oboInOwl:id>GAZ:00061873</oboInOwl:id>
        <rdfs:label>Kremnica Mountains</rdfs:label>
    </owl:NamedIndividual>
    


    <!-- http://purl.obolibrary.org/obo/GAZ_00061874 -->

    <owl:NamedIndividual rdf:about="http://purl.obolibrary.org/obo/GAZ_00061874">
        <obo:RO_0001025 rdf:resource="http://purl.obolibrary.org/obo/GAZ_00061865"/>
        <oboInOwl:hasOBONamespace>GAZ</oboInOwl:hasOBONamespace>
        <oboInOwl:id>GAZ:00061874</oboInOwl:id>
        <rdfs:label>Zupkovska brazda</rdfs:label>
    </owl:NamedIndividual>
    


    <!-- http://purl.obolibrary.org/obo/GAZ_00061875 -->

    <owl:NamedIndividual rdf:about="http://purl.obolibrary.org/obo/GAZ_00061875">
        <obo:RO_0001025 rdf:resource="http://purl.obolibrary.org/obo/GAZ_00061865"/>
        <oboInOwl:hasOBONamespace>GAZ</oboInOwl:hasOBONamespace>
        <oboInOwl:id>GAZ:00061875</oboInOwl:id>
        <rdfs:label>Nizky Vtacnik</rdfs:label>
    </owl:NamedIndividual>
    


    <!-- http://purl.obolibrary.org/obo/GAZ_00061876 -->

    <owl:NamedIndividual rdf:about="http://purl.obolibrary.org/obo/GAZ_00061876">
        <obo:RO_0001025 rdf:resource="http://purl.obolibrary.org/obo/GAZ_00061865"/>
        <oboInOwl:hasOBONamespace>GAZ</oboInOwl:hasOBONamespace>
        <oboInOwl:id>GAZ:00061876</oboInOwl:id>
        <rdfs:label>Raj</rdfs:label>
    </owl:NamedIndividual>
    


    <!-- http://purl.obolibrary.org/obo/GAZ_00061877 -->

    <owl:NamedIndividual rdf:about="http://purl.obolibrary.org/obo/GAZ_00061877">
        <obo:RO_0001025 rdf:resource="http://purl.obolibrary.org/obo/GAZ_00061865"/>
        <oboInOwl:hasOBONamespace>GAZ</oboInOwl:hasOBONamespace>
        <oboInOwl:id>GAZ:00061877</oboInOwl:id>
        <rdfs:label>Vysoky Vtannik</rdfs:label>
    </owl:NamedIndividual>
    


    <!-- http://purl.obolibrary.org/obo/GAZ_00061878 -->

    <owl:NamedIndividual rdf:about="http://purl.obolibrary.org/obo/GAZ_00061878">
        <obo:RO_0001025 rdf:resource="http://purl.obolibrary.org/obo/GAZ_00061873"/>
        <obo:IAO_0000115>The S region of the Kremnica Mountains.</obo:IAO_0000115>
        <oboInOwl:hasOBONamespace>GAZ</oboInOwl:hasOBONamespace>
        <oboInOwl:id>GAZ:00061878</oboInOwl:id>
        <rdfs:label>Turovske predhorie</rdfs:label>
    </owl:NamedIndividual>
    


    <!-- http://purl.obolibrary.org/obo/GAZ_00061879 -->

    <owl:NamedIndividual rdf:about="http://purl.obolibrary.org/obo/GAZ_00061879">
        <obo:RO_0001025 rdf:resource="http://purl.obolibrary.org/obo/GAZ_00061873"/>
        <obo:IAO_0000115>The SW region of the Kremnica Mountains.</obo:IAO_0000115>
        <oboInOwl:hasOBONamespace>GAZ</oboInOwl:hasOBONamespace>
        <oboInOwl:id>GAZ:00061879</oboInOwl:id>
        <rdfs:label>Jastrabska vrchovina</rdfs:label>
    </owl:NamedIndividual>
    


    <!-- http://purl.obolibrary.org/obo/GAZ_00061880 -->

    <owl:NamedIndividual rdf:about="http://purl.obolibrary.org/obo/GAZ_00061880">
        <obo:RO_0001025 rdf:resource="http://purl.obolibrary.org/obo/GAZ_00061873"/>
        <obo:IAO_0000115>The E region of the Kremnica Mountains.</obo:IAO_0000115>
        <oboInOwl:hasOBONamespace>GAZ</oboInOwl:hasOBONamespace>
        <oboInOwl:id>GAZ:00061880</oboInOwl:id>
        <rdfs:label>Malachovske predhorie</rdfs:label>
    </owl:NamedIndividual>
    


    <!-- http://purl.obolibrary.org/obo/GAZ_00061881 -->

    <owl:NamedIndividual rdf:about="http://purl.obolibrary.org/obo/GAZ_00061881">
        <obo:RO_0001025 rdf:resource="http://purl.obolibrary.org/obo/GAZ_00061873"/>
        <obo:IAO_0000115>The N and central regions of the Kremnica Mountains.</obo:IAO_0000115>
        <oboInOwl:hasOBONamespace>GAZ</oboInOwl:hasOBONamespace>
        <oboInOwl:id>GAZ:00061881</oboInOwl:id>
        <rdfs:label>Flochovsky chrbat</rdfs:label>
    </owl:NamedIndividual>
    


    <!-- http://purl.obolibrary.org/obo/GAZ_00061882 -->

    <owl:NamedIndividual rdf:about="http://purl.obolibrary.org/obo/GAZ_00061882">
        <obo:RO_0001025 rdf:resource="http://purl.obolibrary.org/obo/GAZ_00061873"/>
        <obo:IAO_0000115>The NW region of the Kremnica Mountains.</obo:IAO_0000115>
        <oboInOwl:hasOBONamespace>GAZ</oboInOwl:hasOBONamespace>
        <oboInOwl:id>GAZ:00061882</oboInOwl:id>
        <rdfs:label>Kunesovska hornatina</rdfs:label>
    </owl:NamedIndividual>
    


    <!-- http://purl.obolibrary.org/obo/GAZ_00061883 -->

    <owl:NamedIndividual rdf:about="http://purl.obolibrary.org/obo/GAZ_00061883">
        <obo:RO_0001025 rdf:resource="http://purl.obolibrary.org/obo/GAZ_00061694"/>
        <obo:IAO_0000115>A part of the Inner Western Carpathians.</obo:IAO_0000115>
        <oboInOwl:hasOBONamespace>GAZ</oboInOwl:hasOBONamespace>
        <oboInOwl:id>GAZ:00061883</oboInOwl:id>
        <rdfs:label>Lucenec-Kosice Depression</rdfs:label>
    </owl:NamedIndividual>
    


    <!-- http://purl.obolibrary.org/obo/GAZ_00061884 -->

    <owl:NamedIndividual rdf:about="http://purl.obolibrary.org/obo/GAZ_00061884">
        <obo:RO_0001025 rdf:resource="http://purl.obolibrary.org/obo/GAZ_00061883"/>
        <oboInOwl:hasOBONamespace>GAZ</oboInOwl:hasOBONamespace>
        <oboInOwl:id>GAZ:00061884</oboInOwl:id>
        <rdfs:label>Central Ipoly Basin</rdfs:label>
    </owl:NamedIndividual>
    


    <!-- http://purl.obolibrary.org/obo/GAZ_00061885 -->

    <owl:NamedIndividual rdf:about="http://purl.obolibrary.org/obo/GAZ_00061885">
        <obo:RO_0001025 rdf:resource="http://purl.obolibrary.org/obo/GAZ_00061883"/>
        <oboInOwl:hasOBONamespace>GAZ</oboInOwl:hasOBONamespace>
        <oboInOwl:id>GAZ:00061885</oboInOwl:id>
        <rdfs:label>Borsod Hills</rdfs:label>
    </owl:NamedIndividual>
    


    <!-- http://purl.obolibrary.org/obo/GAZ_00061886 -->

    <owl:NamedIndividual rdf:about="http://purl.obolibrary.org/obo/GAZ_00061886">
        <obo:RO_0001025 rdf:resource="http://purl.obolibrary.org/obo/GAZ_00061883"/>
        <oboInOwl:hasOBONamespace>GAZ</oboInOwl:hasOBONamespace>
        <oboInOwl:id>GAZ:00061886</oboInOwl:id>
        <rdfs:label>Hernad-Valley Basin</rdfs:label>
    </owl:NamedIndividual>
    


    <!-- http://purl.obolibrary.org/obo/GAZ_00061887 -->

    <owl:NamedIndividual rdf:about="http://purl.obolibrary.org/obo/GAZ_00061887">
        <obo:RO_0001025 rdf:resource="http://purl.obolibrary.org/obo/GAZ_00061883"/>
        <oboInOwl:hasOBONamespace>GAZ</oboInOwl:hasOBONamespace>
        <oboInOwl:id>GAZ:00061887</oboInOwl:id>
        <rdfs:label>Southern Slovak Basin</rdfs:label>
    </owl:NamedIndividual>
    


    <!-- http://purl.obolibrary.org/obo/GAZ_00061888 -->

    <owl:NamedIndividual rdf:about="http://purl.obolibrary.org/obo/GAZ_00061888">
        <obo:RO_0001025 rdf:resource="http://purl.obolibrary.org/obo/GAZ_00061883"/>
        <oboInOwl:hasOBONamespace>GAZ</oboInOwl:hasOBONamespace>
        <oboInOwl:id>GAZ:00061888</oboInOwl:id>
        <rdfs:label>Bodva Hills</rdfs:label>
    </owl:NamedIndividual>
    


    <!-- http://purl.obolibrary.org/obo/GAZ_00061889 -->

    <owl:NamedIndividual rdf:about="http://purl.obolibrary.org/obo/GAZ_00061889">
        <obo:RO_0001025 rdf:resource="http://purl.obolibrary.org/obo/GAZ_00061883"/>
        <oboInOwl:hasOBONamespace>GAZ</oboInOwl:hasOBONamespace>
        <oboInOwl:id>GAZ:00061889</oboInOwl:id>
        <rdfs:label>Kosice Basin</rdfs:label>
    </owl:NamedIndividual>
    


    <!-- http://purl.obolibrary.org/obo/GAZ_00061890 -->

    <owl:NamedIndividual rdf:about="http://purl.obolibrary.org/obo/GAZ_00061890">
        <obo:RO_0001025 rdf:resource="http://purl.obolibrary.org/obo/GAZ_00061689"/>
        <obo:IAO_0000115>A section of the Carpathian Mountains in northeastern Hungary. Much of the area is included in the Bukk National Park.</obo:IAO_0000115>
        <oboInOwl:hasOBONamespace>GAZ</oboInOwl:hasOBONamespace>
        <oboInOwl:id>GAZ:00061890</oboInOwl:id>
        <rdfs:label>Bukk Mountains</rdfs:label>
    </owl:NamedIndividual>
    


    <!-- http://purl.obolibrary.org/obo/GAZ_00061891 -->

    <owl:NamedIndividual rdf:about="http://purl.obolibrary.org/obo/GAZ_00061891">
        <obo:RO_0001025 rdf:resource="http://purl.obolibrary.org/obo/GAZ_00061689"/>
        <oboInOwl:hasOBONamespace>GAZ</oboInOwl:hasOBONamespace>
        <oboInOwl:id>GAZ:00061891</oboInOwl:id>
        <rdfs:label>Cserehat Hills</rdfs:label>
    </owl:NamedIndividual>
    


    <!-- http://purl.obolibrary.org/obo/GAZ_00061892 -->

    <owl:NamedIndividual rdf:about="http://purl.obolibrary.org/obo/GAZ_00061892">
        <obo:RO_0001025 rdf:resource="http://purl.obolibrary.org/obo/GAZ_00061689"/>
        <oboInOwl:hasOBONamespace>GAZ</oboInOwl:hasOBONamespace>
        <oboInOwl:id>GAZ:00061892</oboInOwl:id>
        <rdfs:label>Burda</rdfs:label>
    </owl:NamedIndividual>
    


    <!-- http://purl.obolibrary.org/obo/GAZ_00061893 -->

    <owl:NamedIndividual rdf:about="http://purl.obolibrary.org/obo/GAZ_00061893">
        <obo:RO_0001025 rdf:resource="http://purl.obolibrary.org/obo/GAZ_00061689"/>
        <obo:IAO_0000115>A mountain range in northern Hungary, between to the towns Gyongyos and Eger. The Matra Mountains are part of the Northern Mountain Range and belong by origin to the largest young volcanic zone of Europe. They are situated between the valleys of River Tarna and River Zagyva.</obo:IAO_0000115>
        <oboInOwl:hasOBONamespace>GAZ</oboInOwl:hasOBONamespace>
        <oboInOwl:id>GAZ:00061893</oboInOwl:id>
        <rdfs:label>Matra Mountains</rdfs:label>
    </owl:NamedIndividual>
    


    <!-- http://purl.obolibrary.org/obo/GAZ_00061894 -->

    <owl:NamedIndividual rdf:about="http://purl.obolibrary.org/obo/GAZ_00061894">
        <obo:RO_0001025 rdf:resource="http://purl.obolibrary.org/obo/GAZ_00061689"/>
        <oboInOwl:hasOBONamespace>GAZ</oboInOwl:hasOBONamespace>
        <oboInOwl:id>GAZ:00061894</oboInOwl:id>
        <rdfs:label>Cerova Highlands</rdfs:label>
    </owl:NamedIndividual>
    


    <!-- http://purl.obolibrary.org/obo/GAZ_00061895 -->

    <owl:NamedIndividual rdf:about="http://purl.obolibrary.org/obo/GAZ_00061895">
        <obo:RO_0001025 rdf:resource="http://purl.obolibrary.org/obo/GAZ_00061689"/>
        <oboInOwl:hasOBONamespace>GAZ</oboInOwl:hasOBONamespace>
        <oboInOwl:id>GAZ:00061895</oboInOwl:id>
        <rdfs:label>Godollo Hills</rdfs:label>
    </owl:NamedIndividual>
    


    <!-- http://purl.obolibrary.org/obo/GAZ_00061896 -->

    <owl:NamedIndividual rdf:about="http://purl.obolibrary.org/obo/GAZ_00061896">
        <obo:RO_0001025 rdf:resource="http://purl.obolibrary.org/obo/GAZ_00061689"/>
        <oboInOwl:hasOBONamespace>GAZ</oboInOwl:hasOBONamespace>
        <oboInOwl:id>GAZ:00061896</oboInOwl:id>
        <rdfs:label>Cserhat Mountains</rdfs:label>
    </owl:NamedIndividual>
    


    <!-- http://purl.obolibrary.org/obo/GAZ_00061897 -->

    <owl:NamedIndividual rdf:about="http://purl.obolibrary.org/obo/GAZ_00061897">
        <obo:RO_0001025 rdf:resource="http://purl.obolibrary.org/obo/GAZ_00061893"/>
        <obo:IAO_0000115>The plateau of Matraberc (Matra ridge) and the groups of the volcanic cones of Galyateto and Kekesteto.</obo:IAO_0000115>
        <oboInOwl:hasOBONamespace>GAZ</oboInOwl:hasOBONamespace>
        <oboInOwl:id>GAZ:00061897</oboInOwl:id>
        <rdfs:label>Central aatra</rdfs:label>
    </owl:NamedIndividual>
    


    <!-- http://purl.obolibrary.org/obo/GAZ_00061898 -->

    <owl:NamedIndividual rdf:about="http://purl.obolibrary.org/obo/GAZ_00061898">
        <obo:RO_0001025 rdf:resource="http://purl.obolibrary.org/obo/GAZ_00061893"/>
        <oboInOwl:hasOBONamespace>GAZ</oboInOwl:hasOBONamespace>
        <oboInOwl:id>GAZ:00061898</oboInOwl:id>
        <rdfs:label>Nagy-volgy</rdfs:label>
    </owl:NamedIndividual>
    


    <!-- http://purl.obolibrary.org/obo/GAZ_00061899 -->

    <owl:NamedIndividual rdf:about="http://purl.obolibrary.org/obo/GAZ_00061899">
        <obo:RO_0001025 rdf:resource="http://purl.obolibrary.org/obo/GAZ_00061890"/>
        <obo:IAO_0000115>A national park in the Bukk Mountains of Northern Hungary, near Miskolc. Established in 1976.</obo:IAO_0000115>
        <oboInOwl:hasOBONamespace>GAZ</oboInOwl:hasOBONamespace>
        <oboInOwl:id>GAZ:00061899</oboInOwl:id>
        <rdfs:label>Bukk National Park</rdfs:label>
    </owl:NamedIndividual>
    


    <!-- http://purl.obolibrary.org/obo/GAZ_00061900 -->

    <owl:NamedIndividual rdf:about="http://purl.obolibrary.org/obo/GAZ_00061900">
        <obo:RO_0001025 rdf:resource="http://purl.obolibrary.org/obo/GAZ_00061698"/>
        <obo:IAO_0000115>A subprovince of the Carpathian Mountains.</obo:IAO_0000115>
        <oboInOwl:hasOBONamespace>GAZ</oboInOwl:hasOBONamespace>
        <oboInOwl:id>GAZ:00061900</oboInOwl:id>
        <rdfs:label>Outer Eastern Carpathians</rdfs:label>
    </owl:NamedIndividual>
    


    <!-- http://purl.obolibrary.org/obo/GAZ_00061901 -->

    <owl:NamedIndividual rdf:about="http://purl.obolibrary.org/obo/GAZ_00061901">
        <obo:RO_0001025 rdf:resource="http://purl.obolibrary.org/obo/GAZ_00061698"/>
        <obo:IAO_0000115>A subprovince of the Carpathian Mountains.</obo:IAO_0000115>
        <oboInOwl:hasOBONamespace>GAZ</oboInOwl:hasOBONamespace>
        <oboInOwl:id>GAZ:00061901</oboInOwl:id>
        <rdfs:label>Inner Eastern Carpathians</rdfs:label>
    </owl:NamedIndividual>
    


    <!-- http://purl.obolibrary.org/obo/GAZ_00061902 -->

    <owl:NamedIndividual rdf:about="http://purl.obolibrary.org/obo/GAZ_00061902">
        <obo:RO_0001025 rdf:resource="http://purl.obolibrary.org/obo/GAZ_00061900"/>
        <obo:IAO_0000115>A mountain range in the extreme south-east of Poland, extending into Ukraine and Slovakia.</obo:IAO_0000115>
        <oboInOwl:hasOBONamespace>GAZ</oboInOwl:hasOBONamespace>
        <oboInOwl:id>GAZ:00061902</oboInOwl:id>
        <rdfs:label>Eastern Beskids (Polish)</rdfs:label>
    </owl:NamedIndividual>
    


    <!-- http://purl.obolibrary.org/obo/GAZ_00061903 -->

    <owl:NamedIndividual rdf:about="http://purl.obolibrary.org/obo/GAZ_00061903">
        <obo:RO_0001025 rdf:resource="http://purl.obolibrary.org/obo/GAZ_00061900"/>
        <oboInOwl:hasOBONamespace>GAZ</oboInOwl:hasOBONamespace>
        <oboInOwl:id>GAZ:00061903</oboInOwl:id>
        <rdfs:label>Lower Beskids</rdfs:label>
    </owl:NamedIndividual>
    


    <!-- http://purl.obolibrary.org/obo/GAZ_00061904 -->

    <owl:NamedIndividual rdf:about="http://purl.obolibrary.org/obo/GAZ_00061904">
        <obo:RO_0001025 rdf:resource="http://purl.obolibrary.org/obo/GAZ_00061900"/>
        <oboInOwl:hasOBONamespace>GAZ</oboInOwl:hasOBONamespace>
        <oboInOwl:id>GAZ:00061904</oboInOwl:id>
        <rdfs:label>Central Beskidian Piedmont</rdfs:label>
    </owl:NamedIndividual>
    


    <!-- http://purl.obolibrary.org/obo/GAZ_00061905 -->

    <owl:NamedIndividual rdf:about="http://purl.obolibrary.org/obo/GAZ_00061905">
        <obo:RO_0001025 rdf:resource="http://purl.obolibrary.org/obo/GAZ_00061900"/>
        <oboInOwl:hasOBONamespace>GAZ</oboInOwl:hasOBONamespace>
        <oboInOwl:id>GAZ:00061905</oboInOwl:id>
        <rdfs:label>Moldavian-Muntenian Carpathians</rdfs:label>
    </owl:NamedIndividual>
    


    <!-- http://purl.obolibrary.org/obo/GAZ_00061906 -->

    <owl:NamedIndividual rdf:about="http://purl.obolibrary.org/obo/GAZ_00061906">
        <obo:RO_0001025 rdf:resource="http://purl.obolibrary.org/obo/GAZ_00061905"/>
        <oboInOwl:hasOBONamespace>GAZ</oboInOwl:hasOBONamespace>
        <oboInOwl:id>GAZ:00061906</oboInOwl:id>
        <rdfs:label>Ciucas Mountains</rdfs:label>
    </owl:NamedIndividual>
    


    <!-- http://purl.obolibrary.org/obo/GAZ_00061907 -->

    <owl:NamedIndividual rdf:about="http://purl.obolibrary.org/obo/GAZ_00061907">
        <obo:RO_0001025 rdf:resource="http://purl.obolibrary.org/obo/GAZ_00061905"/>
        <oboInOwl:hasOBONamespace>GAZ</oboInOwl:hasOBONamespace>
        <oboInOwl:id>GAZ:00061907</oboInOwl:id>
        <rdfs:label>Comanesti Depression</rdfs:label>
    </owl:NamedIndividual>
    


    <!-- http://purl.obolibrary.org/obo/GAZ_00061908 -->

    <owl:NamedIndividual rdf:about="http://purl.obolibrary.org/obo/GAZ_00061908">
        <obo:RO_0001025 rdf:resource="http://purl.obolibrary.org/obo/GAZ_00061905"/>
        <oboInOwl:hasOBONamespace>GAZ</oboInOwl:hasOBONamespace>
        <oboInOwl:id>GAZ:00061908</oboInOwl:id>
        <rdfs:label>Ciuc Mountains</rdfs:label>
    </owl:NamedIndividual>
    


    <!-- http://purl.obolibrary.org/obo/GAZ_00061909 -->

    <owl:NamedIndividual rdf:about="http://purl.obolibrary.org/obo/GAZ_00061909">
        <obo:RO_0001025 rdf:resource="http://purl.obolibrary.org/obo/GAZ_00061912"/>
        <oboInOwl:hasOBONamespace>GAZ</oboInOwl:hasOBONamespace>
        <oboInOwl:id>GAZ:00061909</oboInOwl:id>
        <rdfs:label>Feredeu Ridge</rdfs:label>
    </owl:NamedIndividual>
    


    <!-- http://purl.obolibrary.org/obo/GAZ_00061910 -->

    <owl:NamedIndividual rdf:about="http://purl.obolibrary.org/obo/GAZ_00061910">
        <obo:RO_0001025 rdf:resource="http://purl.obolibrary.org/obo/GAZ_00061905"/>
        <oboInOwl:hasOBONamespace>GAZ</oboInOwl:hasOBONamespace>
        <oboInOwl:id>GAZ:00061910</oboInOwl:id>
        <rdfs:label>Nemira Mountains</rdfs:label>
    </owl:NamedIndividual>
    


    <!-- http://purl.obolibrary.org/obo/GAZ_00061911 -->

    <owl:NamedIndividual rdf:about="http://purl.obolibrary.org/obo/GAZ_00061911">
        <obo:RO_0001025 rdf:resource="http://purl.obolibrary.org/obo/GAZ_00061905"/>
        <obo:IAO_0000115>A mountain range in the Carpathian Mountains of eastern Vrancea county in Romania.</obo:IAO_0000115>
        <oboInOwl:hasOBONamespace>GAZ</oboInOwl:hasOBONamespace>
        <oboInOwl:id>GAZ:00061911</oboInOwl:id>
        <rdfs:label>Vrancea Mountains</rdfs:label>
    </owl:NamedIndividual>
    


    <!-- http://purl.obolibrary.org/obo/GAZ_00061912 -->

    <owl:NamedIndividual rdf:about="http://purl.obolibrary.org/obo/GAZ_00061912">
        <obo:RO_0001025 rdf:resource="http://purl.obolibrary.org/obo/GAZ_00061905"/>
        <oboInOwl:hasOBONamespace>GAZ</oboInOwl:hasOBONamespace>
        <oboInOwl:id>GAZ:00061912</oboInOwl:id>
        <rdfs:label>Bucovina Ridges</rdfs:label>
    </owl:NamedIndividual>
    


    <!-- http://purl.obolibrary.org/obo/GAZ_00061913 -->

    <owl:NamedIndividual rdf:about="http://purl.obolibrary.org/obo/GAZ_00061913">
        <obo:RO_0001025 rdf:resource="http://purl.obolibrary.org/obo/GAZ_00061905"/>
        <obo:IAO_0000115>A mountain range.</obo:IAO_0000115>
        <oboInOwl:hasOBONamespace>GAZ</oboInOwl:hasOBONamespace>
        <oboInOwl:id>GAZ:00061913</oboInOwl:id>
        <rdfs:label>Stanisoara Mountains</rdfs:label>
    </owl:NamedIndividual>
    


    <!-- http://purl.obolibrary.org/obo/GAZ_00061914 -->

    <owl:NamedIndividual rdf:about="http://purl.obolibrary.org/obo/GAZ_00061914">
        <obo:RO_0001025 rdf:resource="http://purl.obolibrary.org/obo/GAZ_00061905"/>
        <oboInOwl:hasOBONamespace>GAZ</oboInOwl:hasOBONamespace>
        <oboInOwl:id>GAZ:00061914</oboInOwl:id>
        <rdfs:label>Tarcau Mountains</rdfs:label>
    </owl:NamedIndividual>
    


    <!-- http://purl.obolibrary.org/obo/GAZ_00061915 -->

    <owl:NamedIndividual rdf:about="http://purl.obolibrary.org/obo/GAZ_00061915">
        <obo:RO_0001025 rdf:resource="http://purl.obolibrary.org/obo/GAZ_00061905"/>
        <oboInOwl:hasOBONamespace>GAZ</oboInOwl:hasOBONamespace>
        <oboInOwl:id>GAZ:00061915</oboInOwl:id>
        <rdfs:label>Buzau Mountains</rdfs:label>
    </owl:NamedIndividual>
    


    <!-- http://purl.obolibrary.org/obo/GAZ_00061916 -->

    <owl:NamedIndividual rdf:about="http://purl.obolibrary.org/obo/GAZ_00061916">
        <obo:RO_0001025 rdf:resource="http://purl.obolibrary.org/obo/GAZ_00061908"/>
        <oboInOwl:hasOBONamespace>GAZ</oboInOwl:hasOBONamespace>
        <oboInOwl:id>GAZ:00061916</oboInOwl:id>
        <rdfs:label>Bodoc Mountains</rdfs:label>
    </owl:NamedIndividual>
    


    <!-- http://purl.obolibrary.org/obo/GAZ_00061917 -->

    <owl:NamedIndividual rdf:about="http://purl.obolibrary.org/obo/GAZ_00061917">
        <obo:RO_0001025 rdf:resource="http://purl.obolibrary.org/obo/GAZ_00061902"/>
        <oboInOwl:hasOBONamespace>GAZ</oboInOwl:hasOBONamespace>
        <oboInOwl:id>GAZ:00061917</oboInOwl:id>
        <rdfs:label>Polonynian Ridge</rdfs:label>
    </owl:NamedIndividual>
    


    <!-- http://purl.obolibrary.org/obo/GAZ_00061918 -->

    <owl:NamedIndividual rdf:about="http://purl.obolibrary.org/obo/GAZ_00061918">
        <obo:RO_0001025 rdf:resource="http://purl.obolibrary.org/obo/GAZ_00061902"/>
        <oboInOwl:hasOBONamespace>GAZ</oboInOwl:hasOBONamespace>
        <oboInOwl:id>GAZ:00061918</oboInOwl:id>
        <rdfs:label>Wooded Beskids</rdfs:label>
    </owl:NamedIndividual>
    


    <!-- http://purl.obolibrary.org/obo/GAZ_00061919 -->

    <owl:NamedIndividual rdf:about="http://purl.obolibrary.org/obo/GAZ_00061919">
        <obo:RO_0001025 rdf:resource="http://purl.obolibrary.org/obo/GAZ_00061917"/>
        <oboInOwl:hasOBONamespace>GAZ</oboInOwl:hasOBONamespace>
        <oboInOwl:id>GAZ:00061919</oboInOwl:id>
        <rdfs:label>Polonyna Borzhava</rdfs:label>
    </owl:NamedIndividual>
    


    <!-- http://purl.obolibrary.org/obo/GAZ_00061920 -->

    <owl:NamedIndividual rdf:about="http://purl.obolibrary.org/obo/GAZ_00061920">
        <obo:RO_0001025 rdf:resource="http://purl.obolibrary.org/obo/GAZ_00061917"/>
        <obo:IAO_0000115>The highest mountain range in Western Ukraine in Outer Eastern Carpathians. It is adjacent to the Gorgany range. The major part of the range forms the watershed between the Prut and Tysa River.</obo:IAO_0000115>
        <oboInOwl:hasOBONamespace>GAZ</oboInOwl:hasOBONamespace>
        <oboInOwl:id>GAZ:00061920</oboInOwl:id>
        <rdfs:label>Chornohora</rdfs:label>
    </owl:NamedIndividual>
    


    <!-- http://purl.obolibrary.org/obo/GAZ_00061921 -->

    <owl:NamedIndividual rdf:about="http://purl.obolibrary.org/obo/GAZ_00061921">
        <obo:RO_0001025 rdf:resource="http://purl.obolibrary.org/obo/GAZ_00061917"/>
        <oboInOwl:hasOBONamespace>GAZ</oboInOwl:hasOBONamespace>
        <oboInOwl:id>GAZ:00061921</oboInOwl:id>
        <rdfs:label>Svydovets&apos;</rdfs:label>
    </owl:NamedIndividual>
    


    <!-- http://purl.obolibrary.org/obo/GAZ_00061922 -->

    <owl:NamedIndividual rdf:about="http://purl.obolibrary.org/obo/GAZ_00061922">
        <obo:RO_0001025 rdf:resource="http://purl.obolibrary.org/obo/GAZ_00061917"/>
        <oboInOwl:hasOBONamespace>GAZ</oboInOwl:hasOBONamespace>
        <oboInOwl:id>GAZ:00061922</oboInOwl:id>
        <rdfs:label>Hryniavs&apos;ki hory</rdfs:label>
    </owl:NamedIndividual>
    


    <!-- http://purl.obolibrary.org/obo/GAZ_00061923 -->

    <owl:NamedIndividual rdf:about="http://purl.obolibrary.org/obo/GAZ_00061923">
        <obo:RO_0001025 rdf:resource="http://purl.obolibrary.org/obo/GAZ_00061917"/>
        <oboInOwl:hasOBONamespace>GAZ</oboInOwl:hasOBONamespace>
        <oboInOwl:id>GAZ:00061923</oboInOwl:id>
        <rdfs:label>Red Polonyna</rdfs:label>
    </owl:NamedIndividual>
    


    <!-- http://purl.obolibrary.org/obo/GAZ_00061924 -->

    <owl:NamedIndividual rdf:about="http://purl.obolibrary.org/obo/GAZ_00061924">
        <obo:RO_0001025 rdf:resource="http://purl.obolibrary.org/obo/GAZ_00061917"/>
        <oboInOwl:hasOBONamespace>GAZ</oboInOwl:hasOBONamespace>
        <oboInOwl:id>GAZ:00061924</oboInOwl:id>
        <rdfs:label>Smooth Polonyna</rdfs:label>
    </owl:NamedIndividual>
    


    <!-- http://purl.obolibrary.org/obo/GAZ_00061925 -->

    <owl:NamedIndividual rdf:about="http://purl.obolibrary.org/obo/GAZ_00061925">
        <obo:RO_0001025 rdf:resource="http://purl.obolibrary.org/obo/GAZ_00061918"/>
        <oboInOwl:hasOBONamespace>GAZ</oboInOwl:hasOBONamespace>
        <oboInOwl:id>GAZ:00061925</oboInOwl:id>
        <rdfs:label>Skole Beskids</rdfs:label>
    </owl:NamedIndividual>
    


    <!-- http://purl.obolibrary.org/obo/GAZ_00061926 -->

    <owl:NamedIndividual rdf:about="http://purl.obolibrary.org/obo/GAZ_00061926">
        <obo:RO_0001025 rdf:resource="http://purl.obolibrary.org/obo/GAZ_00061918"/>
        <oboInOwl:hasOBONamespace>GAZ</oboInOwl:hasOBONamespace>
        <oboInOwl:id>GAZ:00061926</oboInOwl:id>
        <rdfs:label>Upper Dniester Beskids</rdfs:label>
    </owl:NamedIndividual>
    


    <!-- http://purl.obolibrary.org/obo/GAZ_00061927 -->

    <owl:NamedIndividual rdf:about="http://purl.obolibrary.org/obo/GAZ_00061927">
        <obo:RO_0001025 rdf:resource="http://purl.obolibrary.org/obo/GAZ_00061918"/>
        <oboInOwl:hasOBONamespace>GAZ</oboInOwl:hasOBONamespace>
        <oboInOwl:id>GAZ:00061927</oboInOwl:id>
        <rdfs:label>Pokutsk-Bucovina Carpathians</rdfs:label>
    </owl:NamedIndividual>
    


    <!-- http://purl.obolibrary.org/obo/GAZ_00061928 -->

    <owl:NamedIndividual rdf:about="http://purl.obolibrary.org/obo/GAZ_00061928">
        <obo:RO_0001025 rdf:resource="http://purl.obolibrary.org/obo/GAZ_00061918"/>
        <obo:IAO_0000115>A mountain range in Western Ukraine in Outer Eastern Carpathians, adjacent to Chornohora range. They are bordered by the Mizunka River and Vyshkovsky Pass in the west and the Prut River and Yablonitsky Pass in the east.</obo:IAO_0000115>
        <oboInOwl:hasOBONamespace>GAZ</oboInOwl:hasOBONamespace>
        <oboInOwl:id>GAZ:00061928</oboInOwl:id>
        <rdfs:label>Gorgany</rdfs:label>
    </owl:NamedIndividual>
    


    <!-- http://purl.obolibrary.org/obo/GAZ_00061929 -->

    <owl:NamedIndividual rdf:about="http://purl.obolibrary.org/obo/GAZ_00061929">
        <obo:RO_0001025 rdf:resource="http://purl.obolibrary.org/obo/GAZ_00061918"/>
        <oboInOwl:hasOBONamespace>GAZ</oboInOwl:hasOBONamespace>
        <oboInOwl:id>GAZ:00061929</oboInOwl:id>
        <rdfs:label>Gory Sanocko-Turczanskie</rdfs:label>
    </owl:NamedIndividual>
    


    <!-- http://purl.obolibrary.org/obo/GAZ_00061930 -->

    <owl:NamedIndividual rdf:about="http://purl.obolibrary.org/obo/GAZ_00061930">
        <obo:RO_0001025 rdf:resource="http://purl.obolibrary.org/obo/GAZ_00061903"/>
        <oboInOwl:hasOBONamespace>GAZ</oboInOwl:hasOBONamespace>
        <oboInOwl:id>GAZ:00061930</oboInOwl:id>
        <rdfs:label>Busov</rdfs:label>
    </owl:NamedIndividual>
    


    <!-- http://purl.obolibrary.org/obo/GAZ_00061931 -->

    <owl:NamedIndividual rdf:about="http://purl.obolibrary.org/obo/GAZ_00061931">
        <obo:RO_0001025 rdf:resource="http://purl.obolibrary.org/obo/GAZ_00061903"/>
        <oboInOwl:hasOBONamespace>GAZ</oboInOwl:hasOBONamespace>
        <oboInOwl:id>GAZ:00061931</oboInOwl:id>
        <rdfs:label>Beskidian Piedmont</rdfs:label>
    </owl:NamedIndividual>
    


    <!-- http://purl.obolibrary.org/obo/GAZ_00061932 -->

    <owl:NamedIndividual rdf:about="http://purl.obolibrary.org/obo/GAZ_00061932">
        <obo:RO_0001025 rdf:resource="http://purl.obolibrary.org/obo/GAZ_00061903"/>
        <obo:IAO_0000115>A mountain range. Is a hilly region in Presov Region, Sanok County and Jaslo County, between Busov, Ondavska vrchovina, Laborecka vrchovina, Beskydske predhorie in Slovakia, Beskid Sadecki, Pogorze Bukowskie and Bieszczady near the river Wisloka, Wislok and Oslawa in Poland.</obo:IAO_0000115>
        <oboInOwl:hasOBONamespace>GAZ</oboInOwl:hasOBONamespace>
        <oboInOwl:id>GAZ:00061932</oboInOwl:id>
        <rdfs:label>Low Beskids</rdfs:label>
    </owl:NamedIndividual>
    


    <!-- http://purl.obolibrary.org/obo/GAZ_00061933 -->

    <owl:NamedIndividual rdf:about="http://purl.obolibrary.org/obo/GAZ_00061933">
        <obo:RO_0001025 rdf:resource="http://purl.obolibrary.org/obo/GAZ_00061903"/>
        <oboInOwl:hasOBONamespace>GAZ</oboInOwl:hasOBONamespace>
        <oboInOwl:id>GAZ:00061933</oboInOwl:id>
        <rdfs:label>Ondava Highlands</rdfs:label>
    </owl:NamedIndividual>
    


    <!-- http://purl.obolibrary.org/obo/GAZ_00061934 -->

    <owl:NamedIndividual rdf:about="http://purl.obolibrary.org/obo/GAZ_00061934">
        <obo:RO_0001025 rdf:resource="http://purl.obolibrary.org/obo/GAZ_00061903"/>
        <oboInOwl:hasOBONamespace>GAZ</oboInOwl:hasOBONamespace>
        <oboInOwl:id>GAZ:00061934</oboInOwl:id>
        <rdfs:label>Laborec Highlands</rdfs:label>
    </owl:NamedIndividual>
    


    <!-- http://purl.obolibrary.org/obo/GAZ_00061935 -->

    <owl:NamedIndividual rdf:about="http://purl.obolibrary.org/obo/GAZ_00061935">
        <obo:RO_0001025 rdf:resource="http://purl.obolibrary.org/obo/GAZ_00061904"/>
        <oboInOwl:hasOBONamespace>GAZ</oboInOwl:hasOBONamespace>
        <oboInOwl:id>GAZ:00061935</oboInOwl:id>
        <rdfs:label>Ciezkowice Piedmont</rdfs:label>
    </owl:NamedIndividual>
    


    <!-- http://purl.obolibrary.org/obo/GAZ_00061936 -->

    <owl:NamedIndividual rdf:about="http://purl.obolibrary.org/obo/GAZ_00061936">
        <obo:RO_0001025 rdf:resource="http://purl.obolibrary.org/obo/GAZ_00061904"/>
        <oboInOwl:hasOBONamespace>GAZ</oboInOwl:hasOBONamespace>
        <oboInOwl:id>GAZ:00061936</oboInOwl:id>
        <rdfs:label>Strzyzow Piedmont</rdfs:label>
    </owl:NamedIndividual>
    


    <!-- http://purl.obolibrary.org/obo/GAZ_00061937 -->

    <owl:NamedIndividual rdf:about="http://purl.obolibrary.org/obo/GAZ_00061937">
        <obo:RO_0001025 rdf:resource="http://purl.obolibrary.org/obo/GAZ_00061904"/>
        <oboInOwl:hasOBONamespace>GAZ</oboInOwl:hasOBONamespace>
        <oboInOwl:id>GAZ:00061937</oboInOwl:id>
        <rdfs:label>Przemysl Piedmont</rdfs:label>
    </owl:NamedIndividual>
    


    <!-- http://purl.obolibrary.org/obo/GAZ_00061938 -->

    <owl:NamedIndividual rdf:about="http://purl.obolibrary.org/obo/GAZ_00061938">
        <obo:RO_0001025 rdf:resource="http://purl.obolibrary.org/obo/GAZ_00061904"/>
        <oboInOwl:hasOBONamespace>GAZ</oboInOwl:hasOBONamespace>
        <oboInOwl:id>GAZ:00061938</oboInOwl:id>
        <rdfs:label>Bukowsko Piedmont</rdfs:label>
    </owl:NamedIndividual>
    


    <!-- http://purl.obolibrary.org/obo/GAZ_00061939 -->

    <owl:NamedIndividual rdf:about="http://purl.obolibrary.org/obo/GAZ_00061939">
        <obo:RO_0001025 rdf:resource="http://purl.obolibrary.org/obo/GAZ_00061904"/>
        <oboInOwl:hasOBONamespace>GAZ</oboInOwl:hasOBONamespace>
        <oboInOwl:id>GAZ:00061939</oboInOwl:id>
        <rdfs:label>Gorlice Depression</rdfs:label>
    </owl:NamedIndividual>
    


    <!-- http://purl.obolibrary.org/obo/GAZ_00061940 -->

    <owl:NamedIndividual rdf:about="http://purl.obolibrary.org/obo/GAZ_00061940">
        <obo:RO_0001025 rdf:resource="http://purl.obolibrary.org/obo/GAZ_00061904"/>
        <oboInOwl:hasOBONamespace>GAZ</oboInOwl:hasOBONamespace>
        <oboInOwl:id>GAZ:00061940</oboInOwl:id>
        <rdfs:label>Roznow Piedmont</rdfs:label>
    </owl:NamedIndividual>
    


    <!-- http://purl.obolibrary.org/obo/GAZ_00061941 -->

    <owl:NamedIndividual rdf:about="http://purl.obolibrary.org/obo/GAZ_00061941">
        <obo:RO_0001025 rdf:resource="http://purl.obolibrary.org/obo/GAZ_00061904"/>
        <oboInOwl:hasOBONamespace>GAZ</oboInOwl:hasOBONamespace>
        <oboInOwl:id>GAZ:00061941</oboInOwl:id>
        <rdfs:label>Jaslo-Krosno Basin</rdfs:label>
    </owl:NamedIndividual>
    


    <!-- http://purl.obolibrary.org/obo/GAZ_00061942 -->

    <owl:NamedIndividual rdf:about="http://purl.obolibrary.org/obo/GAZ_00061942">
        <obo:RO_0001025 rdf:resource="http://purl.obolibrary.org/obo/GAZ_00061904"/>
        <oboInOwl:hasOBONamespace>GAZ</oboInOwl:hasOBONamespace>
        <oboInOwl:id>GAZ:00061942</oboInOwl:id>
        <rdfs:label>Dynow Piedmont</rdfs:label>
    </owl:NamedIndividual>
    


    <!-- http://purl.obolibrary.org/obo/GAZ_00061943 -->

    <owl:NamedIndividual rdf:about="http://purl.obolibrary.org/obo/GAZ_00061943">
        <obo:RO_0001025 rdf:resource="http://purl.obolibrary.org/obo/GAZ_00061904"/>
        <oboInOwl:hasOBONamespace>GAZ</oboInOwl:hasOBONamespace>
        <oboInOwl:id>GAZ:00061943</oboInOwl:id>
        <rdfs:label>Jaslo Piedmont</rdfs:label>
    </owl:NamedIndividual>
    


    <!-- http://purl.obolibrary.org/obo/GAZ_00061944 -->

    <owl:NamedIndividual rdf:about="http://purl.obolibrary.org/obo/GAZ_00061944">
        <obo:RO_0001025 rdf:resource="http://purl.obolibrary.org/obo/GAZ_00061918"/>
        <obo:IAO_0000115>A part of the Carpathian Mountains. The mountain range is situated between the Lupkow Pass (640 m) and the Vyshkovskyi Pass (933 m).</obo:IAO_0000115>
        <oboInOwl:hasOBONamespace>GAZ</oboInOwl:hasOBONamespace>
        <oboInOwl:id>GAZ:00061944</oboInOwl:id>
        <rdfs:label>Bieszczady</rdfs:label>
    </owl:NamedIndividual>
    


    <!-- http://purl.obolibrary.org/obo/GAZ_00061945 -->

    <owl:NamedIndividual rdf:about="http://purl.obolibrary.org/obo/GAZ_00061945">
        <obo:RO_0001025 rdf:resource="http://purl.obolibrary.org/obo/GAZ_00061918"/>
        <obo:RO_0001025 rdf:resource="http://purl.obolibrary.org/obo/GAZ_00471827"/>
        <obo:IAO_0000115>A mountain range. Located in the Presov Region near the borders with Poland (Bieszczady) and Ukraine, and adjacent to the Laborec Highlands.</obo:IAO_0000115>
        <oboInOwl:hasOBONamespace>GAZ</oboInOwl:hasOBONamespace>
        <oboInOwl:id>GAZ:00061945</oboInOwl:id>
        <rdfs:label>Bukovske vrchy</rdfs:label>
    </owl:NamedIndividual>
    


    <!-- http://purl.obolibrary.org/obo/GAZ_00061946 -->

    <owl:NamedIndividual rdf:about="http://purl.obolibrary.org/obo/GAZ_00061946">
        <obo:RO_0001025 rdf:resource="http://purl.obolibrary.org/obo/GAZ_00061945"/>
        <obo:IAO_0000115>A national park in north eastern Slovakia at the Polish and Ukrainian borders, in the Bukovske vrchy mountain range, which belongs to the Eastern Carpathians. Established 1997-10-01.</obo:IAO_0000115>
        <oboInOwl:hasOBONamespace>GAZ</oboInOwl:hasOBONamespace>
        <oboInOwl:id>GAZ:00061946</oboInOwl:id>
        <rdfs:label>Poloniny National Park</rdfs:label>
    </owl:NamedIndividual>
    


    <!-- http://purl.obolibrary.org/obo/GAZ_00061947 -->

    <owl:NamedIndividual rdf:about="http://purl.obolibrary.org/obo/GAZ_00061947">
        <obo:RO_0001025 rdf:resource="http://purl.obolibrary.org/obo/GAZ_00061944"/>
        <obo:IAO_0000115>A national park located in the very south-east corner of the country, along the borders with Slovakia and the Ukraine, in the Subcarpathian Voivodship. The Park was created in 1973, but has since then been enlarged four times. The last enlargements took place in 1996 and 1999, when the Park incorporated the former villages of Bukowiec, Beniowa, Carynskie in 1996, and in 1999 the former villages of Dzwiniacz, Tarnawa and Sokoliki.</obo:IAO_0000115>
        <oboInOwl:hasOBONamespace>GAZ</oboInOwl:hasOBONamespace>
        <oboInOwl:id>GAZ:00061947</oboInOwl:id>
        <rdfs:label>Bieszczadzki Park Narodowy</rdfs:label>
    </owl:NamedIndividual>
    


    <!-- http://purl.obolibrary.org/obo/GAZ_00061948 -->

    <owl:NamedIndividual rdf:about="http://purl.obolibrary.org/obo/GAZ_00061948">
        <obo:RO_0001025 rdf:resource="http://purl.obolibrary.org/obo/GAZ_00061917"/>
        <oboInOwl:hasOBONamespace>GAZ</oboInOwl:hasOBONamespace>
        <oboInOwl:id>GAZ:00061948</oboInOwl:id>
        <rdfs:label>Polonyna Kuk</rdfs:label>
    </owl:NamedIndividual>
    


    <!-- http://purl.obolibrary.org/obo/GAZ_00061949 -->

    <owl:NamedIndividual rdf:about="http://purl.obolibrary.org/obo/GAZ_00061949">
        <obo:RO_0001025 rdf:resource="http://purl.obolibrary.org/obo/GAZ_00061912"/>
        <oboInOwl:hasOBONamespace>GAZ</oboInOwl:hasOBONamespace>
        <oboInOwl:id>GAZ:00061949</oboInOwl:id>
        <rdfs:label>Obcina Mare</rdfs:label>
    </owl:NamedIndividual>
    


    <!-- http://purl.obolibrary.org/obo/GAZ_00061950 -->

    <owl:NamedIndividual rdf:about="http://purl.obolibrary.org/obo/GAZ_00061950">
        <obo:RO_0001025 rdf:resource="http://purl.obolibrary.org/obo/GAZ_00061905"/>
        <oboInOwl:hasOBONamespace>GAZ</oboInOwl:hasOBONamespace>
        <oboInOwl:id>GAZ:00061950</oboInOwl:id>
        <rdfs:label>Barsa Mountains</rdfs:label>
    </owl:NamedIndividual>
    


    <!-- http://purl.obolibrary.org/obo/GAZ_00061951 -->

    <owl:NamedIndividual rdf:about="http://purl.obolibrary.org/obo/GAZ_00061951">
        <obo:RO_0001025 rdf:resource="http://purl.obolibrary.org/obo/GAZ_00061901"/>
        <oboInOwl:hasOBONamespace>GAZ</oboInOwl:hasOBONamespace>
        <oboInOwl:id>GAZ:00061951</oboInOwl:id>
        <rdfs:label>Bistrita Mountains</rdfs:label>
    </owl:NamedIndividual>
    


    <!-- http://purl.obolibrary.org/obo/GAZ_00061952 -->

    <owl:NamedIndividual rdf:about="http://purl.obolibrary.org/obo/GAZ_00061952">
        <obo:RO_0001025 rdf:resource="http://purl.obolibrary.org/obo/GAZ_00061901"/>
        <oboInOwl:hasOBONamespace>GAZ</oboInOwl:hasOBONamespace>
        <oboInOwl:id>GAZ:00061952</oboInOwl:id>
        <rdfs:label>Giurgeu-Brasov Depression</rdfs:label>
    </owl:NamedIndividual>
    


    <!-- http://purl.obolibrary.org/obo/GAZ_00061953 -->

    <owl:NamedIndividual rdf:about="http://purl.obolibrary.org/obo/GAZ_00061953">
        <obo:RO_0001025 rdf:resource="http://purl.obolibrary.org/obo/GAZ_00061901"/>
        <oboInOwl:hasOBONamespace>GAZ</oboInOwl:hasOBONamespace>
        <oboInOwl:id>GAZ:00061953</oboInOwl:id>
        <rdfs:label>Vihorlat-Gutin Area</rdfs:label>
    </owl:NamedIndividual>
    


    <!-- http://purl.obolibrary.org/obo/GAZ_00061954 -->

    <owl:NamedIndividual rdf:about="http://purl.obolibrary.org/obo/GAZ_00061954">
        <obo:RO_0001025 rdf:resource="http://purl.obolibrary.org/obo/GAZ_00061901"/>
        <oboInOwl:hasOBONamespace>GAZ</oboInOwl:hasOBONamespace>
        <oboInOwl:id>GAZ:00061954</oboInOwl:id>
        <rdfs:label>Caliman-Harghita Mountains</rdfs:label>
    </owl:NamedIndividual>
    


    <!-- http://purl.obolibrary.org/obo/GAZ_00061955 -->

    <owl:NamedIndividual rdf:about="http://purl.obolibrary.org/obo/GAZ_00061955">
        <obo:RO_0001025 rdf:resource="http://purl.obolibrary.org/obo/GAZ_00061953"/>
        <obo:IAO_0000115>A volcanic mountain range in eastern Slovakia and western Ukraine. A part of the range is listed as a World Heritage Site. Vihorlat is bordered by the Eastern Slovak Lowland (Vychodoslovenska nizina) in the south and the west. The Beskidian Piedmont (Beskydske predhorie) separates Vihorlat from the Bukovske vrchy mountains and Laborecka vrchovina highlands in the north.</obo:IAO_0000115>
        <oboInOwl:hasOBONamespace>GAZ</oboInOwl:hasOBONamespace>
        <oboInOwl:id>GAZ:00061955</oboInOwl:id>
        <rdfs:label>Vihorlat Mountains</rdfs:label>
    </owl:NamedIndividual>
    


    <!-- http://purl.obolibrary.org/obo/GAZ_00061956 -->

    <owl:NamedIndividual rdf:about="http://purl.obolibrary.org/obo/GAZ_00061956">
        <obo:RO_0001025 rdf:resource="http://purl.obolibrary.org/obo/GAZ_00061953"/>
        <oboInOwl:hasOBONamespace>GAZ</oboInOwl:hasOBONamespace>
        <oboInOwl:id>GAZ:00061956</oboInOwl:id>
        <rdfs:label>Oas Mountains</rdfs:label>
    </owl:NamedIndividual>
    


    <!-- http://purl.obolibrary.org/obo/GAZ_00061957 -->

    <owl:NamedIndividual rdf:about="http://purl.obolibrary.org/obo/GAZ_00061957">
        <obo:RO_0001025 rdf:resource="http://purl.obolibrary.org/obo/GAZ_00061953"/>
        <obo:IAO_0000115>A volcanic mountain range located in northern Romania.</obo:IAO_0000115>
        <oboInOwl:hasOBONamespace>GAZ</oboInOwl:hasOBONamespace>
        <oboInOwl:id>GAZ:00061957</oboInOwl:id>
        <rdfs:label>Tibles Mountains</rdfs:label>
    </owl:NamedIndividual>
    


    <!-- http://purl.obolibrary.org/obo/GAZ_00061958 -->

    <owl:NamedIndividual rdf:about="http://purl.obolibrary.org/obo/GAZ_00061958">
        <obo:RO_0001025 rdf:resource="http://purl.obolibrary.org/obo/GAZ_00061953"/>
        <oboInOwl:hasOBONamespace>GAZ</oboInOwl:hasOBONamespace>
        <oboInOwl:id>GAZ:00061958</oboInOwl:id>
        <rdfs:label>Velikyi Dil</rdfs:label>
    </owl:NamedIndividual>
    


    <!-- http://purl.obolibrary.org/obo/GAZ_00061959 -->

    <owl:NamedIndividual rdf:about="http://purl.obolibrary.org/obo/GAZ_00061959">
        <obo:RO_0001025 rdf:resource="http://purl.obolibrary.org/obo/GAZ_00061953"/>
        <oboInOwl:hasOBONamespace>GAZ</oboInOwl:hasOBONamespace>
        <oboInOwl:id>GAZ:00061959</oboInOwl:id>
        <rdfs:label>Oas Depression</rdfs:label>
    </owl:NamedIndividual>
    


    <!-- http://purl.obolibrary.org/obo/GAZ_00061960 -->

    <owl:NamedIndividual rdf:about="http://purl.obolibrary.org/obo/GAZ_00061960">
        <obo:RO_0001025 rdf:resource="http://purl.obolibrary.org/obo/GAZ_00061953"/>
        <oboInOwl:hasOBONamespace>GAZ</oboInOwl:hasOBONamespace>
        <oboInOwl:id>GAZ:00061960</oboInOwl:id>
        <rdfs:label>Tupyi</rdfs:label>
    </owl:NamedIndividual>
    


    <!-- http://purl.obolibrary.org/obo/GAZ_00061961 -->

    <owl:NamedIndividual rdf:about="http://purl.obolibrary.org/obo/GAZ_00061961">
        <obo:RO_0001025 rdf:resource="http://purl.obolibrary.org/obo/GAZ_00061953"/>
        <obo:IAO_0000115>A mountain range in the Inner Eastern Carpathian Mountains of the Maramures in Romania.</obo:IAO_0000115>
        <oboInOwl:hasOBONamespace>GAZ</oboInOwl:hasOBONamespace>
        <oboInOwl:id>GAZ:00061961</oboInOwl:id>
        <rdfs:label>Gutai Mountains</rdfs:label>
    </owl:NamedIndividual>
    


    <!-- http://purl.obolibrary.org/obo/GAZ_00061962 -->

    <owl:NamedIndividual rdf:about="http://purl.obolibrary.org/obo/GAZ_00061962">
        <obo:RO_0001025 rdf:resource="http://purl.obolibrary.org/obo/GAZ_00061951"/>
        <obo:IAO_0000115>A mountain range located in the Eastern Carpathians chain, in Neamt County, in the Moldavia region.</obo:IAO_0000115>
        <oboInOwl:hasOBONamespace>GAZ</oboInOwl:hasOBONamespace>
        <oboInOwl:id>GAZ:00061962</oboInOwl:id>
        <rdfs:label>Ceahlau Massif</rdfs:label>
    </owl:NamedIndividual>
    


    <!-- http://purl.obolibrary.org/obo/GAZ_00061963 -->

    <owl:NamedIndividual rdf:about="http://purl.obolibrary.org/obo/GAZ_00061963">
        <obo:RO_0001025 rdf:resource="http://purl.obolibrary.org/obo/GAZ_00061951"/>
        <obo:IAO_0000115>A mountain range.</obo:IAO_0000115>
        <oboInOwl:hasOBONamespace>GAZ</oboInOwl:hasOBONamespace>
        <oboInOwl:id>GAZ:00061963</oboInOwl:id>
        <rdfs:label>Great Hasmasu Mountains</rdfs:label>
    </owl:NamedIndividual>
    


    <!-- http://purl.obolibrary.org/obo/GAZ_00061964 -->

    <owl:NamedIndividual rdf:about="http://purl.obolibrary.org/obo/GAZ_00061964">
        <obo:RO_0001025 rdf:resource="http://purl.obolibrary.org/obo/GAZ_00061951"/>
        <oboInOwl:hasOBONamespace>GAZ</oboInOwl:hasOBONamespace>
        <oboInOwl:id>GAZ:00061964</oboInOwl:id>
        <rdfs:label>Budacul Massif</rdfs:label>
    </owl:NamedIndividual>
    


    <!-- http://purl.obolibrary.org/obo/GAZ_00061965 -->

    <owl:NamedIndividual rdf:about="http://purl.obolibrary.org/obo/GAZ_00061965">
        <obo:RO_0001025 rdf:resource="http://purl.obolibrary.org/obo/GAZ_00061951"/>
        <oboInOwl:hasOBONamespace>GAZ</oboInOwl:hasOBONamespace>
        <oboInOwl:id>GAZ:00061965</oboInOwl:id>
        <rdfs:label>Giurgeu Mountains</rdfs:label>
    </owl:NamedIndividual>
    


    <!-- http://purl.obolibrary.org/obo/GAZ_00061966 -->

    <owl:NamedIndividual rdf:about="http://purl.obolibrary.org/obo/GAZ_00061966">
        <obo:RO_0001025 rdf:resource="http://purl.obolibrary.org/obo/GAZ_00061951"/>
        <oboInOwl:hasOBONamespace>GAZ</oboInOwl:hasOBONamespace>
        <oboInOwl:id>GAZ:00061966</oboInOwl:id>
        <rdfs:label>Pietrosul Massif</rdfs:label>
    </owl:NamedIndividual>
    


    <!-- http://purl.obolibrary.org/obo/GAZ_00061967 -->

    <owl:NamedIndividual rdf:about="http://purl.obolibrary.org/obo/GAZ_00061967">
        <obo:RO_0001025 rdf:resource="http://purl.obolibrary.org/obo/GAZ_00061951"/>
        <oboInOwl:hasOBONamespace>GAZ</oboInOwl:hasOBONamespace>
        <oboInOwl:id>GAZ:00061967</oboInOwl:id>
        <rdfs:label>Giumalau-Rarau Mountains</rdfs:label>
    </owl:NamedIndividual>
    


    <!-- http://purl.obolibrary.org/obo/GAZ_00061968 -->

    <owl:NamedIndividual rdf:about="http://purl.obolibrary.org/obo/GAZ_00061968">
        <obo:RO_0001025 rdf:resource="http://purl.obolibrary.org/obo/GAZ_00061951"/>
        <oboInOwl:hasOBONamespace>GAZ</oboInOwl:hasOBONamespace>
        <oboInOwl:id>GAZ:00061968</oboInOwl:id>
        <rdfs:label>Dorna Depression</rdfs:label>
    </owl:NamedIndividual>
    


    <!-- http://purl.obolibrary.org/obo/GAZ_00061969 -->

    <owl:NamedIndividual rdf:about="http://purl.obolibrary.org/obo/GAZ_00061969">
        <obo:RO_0001025 rdf:resource="http://purl.obolibrary.org/obo/GAZ_00061951"/>
        <oboInOwl:hasOBONamespace>GAZ</oboInOwl:hasOBONamespace>
        <oboInOwl:id>GAZ:00061969</oboInOwl:id>
        <rdfs:label>Mestecanis Ridge</rdfs:label>
    </owl:NamedIndividual>
    


    <!-- http://purl.obolibrary.org/obo/GAZ_00061970 -->

    <owl:NamedIndividual rdf:about="http://purl.obolibrary.org/obo/GAZ_00061970">
        <obo:RO_0001025 rdf:resource="http://purl.obolibrary.org/obo/GAZ_00061954"/>
        <obo:IAO_0000115>A mountain range.</obo:IAO_0000115>
        <oboInOwl:hasOBONamespace>GAZ</oboInOwl:hasOBONamespace>
        <oboInOwl:id>GAZ:00061970</oboInOwl:id>
        <rdfs:label>Calimani Mountains</rdfs:label>
    </owl:NamedIndividual>
    


    <!-- http://purl.obolibrary.org/obo/GAZ_00061971 -->

    <owl:NamedIndividual rdf:about="http://purl.obolibrary.org/obo/GAZ_00061971">
        <obo:RO_0001025 rdf:resource="http://purl.obolibrary.org/obo/GAZ_00061954"/>
        <oboInOwl:hasOBONamespace>GAZ</oboInOwl:hasOBONamespace>
        <oboInOwl:id>GAZ:00061971</oboInOwl:id>
        <rdfs:label>Bargu Mountains</rdfs:label>
    </owl:NamedIndividual>
    


    <!-- http://purl.obolibrary.org/obo/GAZ_00061972 -->

    <owl:NamedIndividual rdf:about="http://purl.obolibrary.org/obo/GAZ_00061972">
        <obo:RO_0001025 rdf:resource="http://purl.obolibrary.org/obo/GAZ_00061954"/>
        <oboInOwl:hasOBONamespace>GAZ</oboInOwl:hasOBONamespace>
        <oboInOwl:id>GAZ:00061972</oboInOwl:id>
        <rdfs:label>Harghita Mountains</rdfs:label>
    </owl:NamedIndividual>
    


    <!-- http://purl.obolibrary.org/obo/GAZ_00061973 -->

    <owl:NamedIndividual rdf:about="http://purl.obolibrary.org/obo/GAZ_00061973">
        <obo:RO_0001025 rdf:resource="http://purl.obolibrary.org/obo/GAZ_00061954"/>
        <oboInOwl:hasOBONamespace>GAZ</oboInOwl:hasOBONamespace>
        <oboInOwl:id>GAZ:00061973</oboInOwl:id>
        <rdfs:label>Gurghiu Mountains</rdfs:label>
    </owl:NamedIndividual>
    


    <!-- http://purl.obolibrary.org/obo/GAZ_00061974 -->

    <owl:NamedIndividual rdf:about="http://purl.obolibrary.org/obo/GAZ_00061974">
        <obo:RO_0001025 rdf:resource="http://purl.obolibrary.org/obo/GAZ_00061954"/>
        <obo:IAO_0000115>A mountain range.</obo:IAO_0000115>
        <oboInOwl:hasOBONamespace>GAZ</oboInOwl:hasOBONamespace>
        <oboInOwl:id>GAZ:00061974</oboInOwl:id>
        <rdfs:label>Persani Mountains</rdfs:label>
    </owl:NamedIndividual>
    


    <!-- http://purl.obolibrary.org/obo/GAZ_00061975 -->

    <owl:NamedIndividual rdf:about="http://purl.obolibrary.org/obo/GAZ_00061975">
        <obo:RO_0001025 rdf:resource="http://purl.obolibrary.org/obo/GAZ_00061954"/>
        <oboInOwl:hasOBONamespace>GAZ</oboInOwl:hasOBONamespace>
        <oboInOwl:id>GAZ:00061975</oboInOwl:id>
        <rdfs:label>Baraolt Mountains</rdfs:label>
    </owl:NamedIndividual>
    


    <!-- http://purl.obolibrary.org/obo/GAZ_00061976 -->

    <owl:NamedIndividual rdf:about="http://purl.obolibrary.org/obo/GAZ_00061976">
        <obo:RO_0001025 rdf:resource="http://purl.obolibrary.org/obo/GAZ_00061952"/>
        <oboInOwl:hasOBONamespace>GAZ</oboInOwl:hasOBONamespace>
        <oboInOwl:id>GAZ:00061976</oboInOwl:id>
        <rdfs:label>Giurgeu Depression</rdfs:label>
    </owl:NamedIndividual>
    


    <!-- http://purl.obolibrary.org/obo/GAZ_00061977 -->

    <owl:NamedIndividual rdf:about="http://purl.obolibrary.org/obo/GAZ_00061977">
        <obo:RO_0001025 rdf:resource="http://purl.obolibrary.org/obo/GAZ_00061952"/>
        <oboInOwl:hasOBONamespace>GAZ</oboInOwl:hasOBONamespace>
        <oboInOwl:id>GAZ:00061977</oboInOwl:id>
        <rdfs:label>Ciuc Depression</rdfs:label>
    </owl:NamedIndividual>
    


    <!-- http://purl.obolibrary.org/obo/GAZ_00061978 -->

    <owl:NamedIndividual rdf:about="http://purl.obolibrary.org/obo/GAZ_00061978">
        <obo:RO_0001025 rdf:resource="http://purl.obolibrary.org/obo/GAZ_00061952"/>
        <oboInOwl:hasOBONamespace>GAZ</oboInOwl:hasOBONamespace>
        <oboInOwl:id>GAZ:00061978</oboInOwl:id>
        <rdfs:label>Brasov Depression</rdfs:label>
    </owl:NamedIndividual>
    


    <!-- http://purl.obolibrary.org/obo/GAZ_00061979 -->

    <owl:NamedIndividual rdf:about="http://purl.obolibrary.org/obo/GAZ_00061979">
        <obo:RO_0001025 rdf:resource="http://purl.obolibrary.org/obo/GAZ_00061901"/>
        <oboInOwl:hasOBONamespace>GAZ</oboInOwl:hasOBONamespace>
        <oboInOwl:id>GAZ:00061979</oboInOwl:id>
        <rdfs:label>Maramures Mountains</rdfs:label>
    </owl:NamedIndividual>
    


    <!-- http://purl.obolibrary.org/obo/GAZ_00061980 -->

    <owl:NamedIndividual rdf:about="http://purl.obolibrary.org/obo/GAZ_00061980">
        <obo:RO_0001025 rdf:resource="http://purl.obolibrary.org/obo/GAZ_00061901"/>
        <oboInOwl:hasOBONamespace>GAZ</oboInOwl:hasOBONamespace>
        <oboInOwl:id>GAZ:00061980</oboInOwl:id>
        <rdfs:label>Maramures Depression</rdfs:label>
    </owl:NamedIndividual>
    


    <!-- http://purl.obolibrary.org/obo/GAZ_00061981 -->

    <owl:NamedIndividual rdf:about="http://purl.obolibrary.org/obo/GAZ_00061981">
        <obo:RO_0001025 rdf:resource="http://purl.obolibrary.org/obo/GAZ_00061901"/>
        <oboInOwl:hasOBONamespace>GAZ</oboInOwl:hasOBONamespace>
        <oboInOwl:id>GAZ:00061981</oboInOwl:id>
        <rdfs:label>Rodna Mountains</rdfs:label>
    </owl:NamedIndividual>
    


    <!-- http://purl.obolibrary.org/obo/GAZ_00061982 -->

    <owl:NamedIndividual rdf:about="http://purl.obolibrary.org/obo/GAZ_00061982">
        <obo:RO_0001025 rdf:resource="http://purl.obolibrary.org/obo/GAZ_00061901"/>
        <oboInOwl:hasOBONamespace>GAZ</oboInOwl:hasOBONamespace>
        <oboInOwl:id>GAZ:00061982</oboInOwl:id>
        <rdfs:label>Rakhiv Massif</rdfs:label>
    </owl:NamedIndividual>
    


    <!-- http://purl.obolibrary.org/obo/GAZ_00061983 -->

    <owl:NamedIndividual rdf:about="http://purl.obolibrary.org/obo/GAZ_00061983">
        <obo:RO_0001025 rdf:resource="http://purl.obolibrary.org/obo/GAZ_00061711"/>
        <obo:IAO_0000115>Mountains located in central Romania, south of the city Brasov. They are part of the Southern Carpathians group of the Carpathian Mountains.</obo:IAO_0000115>
        <oboInOwl:hasOBONamespace>GAZ</oboInOwl:hasOBONamespace>
        <oboInOwl:id>GAZ:00061983</oboInOwl:id>
        <rdfs:label>Bucegi Mountains</rdfs:label>
    </owl:NamedIndividual>
    


    <!-- http://purl.obolibrary.org/obo/GAZ_00061984 -->

    <owl:NamedIndividual rdf:about="http://purl.obolibrary.org/obo/GAZ_00061984">
        <obo:RO_0001025 rdf:resource="http://purl.obolibrary.org/obo/GAZ_00061953"/>
        <oboInOwl:hasOBONamespace>GAZ</oboInOwl:hasOBONamespace>
        <oboInOwl:id>GAZ:00061984</oboInOwl:id>
        <rdfs:label>Makovytsia</rdfs:label>
    </owl:NamedIndividual>
    


    <!-- http://purl.obolibrary.org/obo/GAZ_00061985 -->

    <owl:NamedIndividual rdf:about="http://purl.obolibrary.org/obo/GAZ_00061985">
        <obo:RO_0001025 rdf:resource="http://purl.obolibrary.org/obo/GAZ_00061711"/>
        <obo:IAO_0000115>Mountains located in central Romania, north of the city Targoviste. They are part of the Southern Carpathians group of the Carpathian Mountains, and have as neighbours the Bucegi Mountains to the east and Piatra Craiului to the west. The Bran Pass separates the Piatra Craiului and Leaota ranges; it was marked by border crossings between Wallachia and Transylvania, and was defended by the Bran Castle.</obo:IAO_0000115>
        <oboInOwl:hasOBONamespace>GAZ</oboInOwl:hasOBONamespace>
        <oboInOwl:id>GAZ:00061985</oboInOwl:id>
        <rdfs:label>Leaota Mountains</rdfs:label>
    </owl:NamedIndividual>
    


    <!-- http://purl.obolibrary.org/obo/GAZ_00061987 -->

    <owl:NamedIndividual rdf:about="http://purl.obolibrary.org/obo/GAZ_00061987">
        <obo:RO_0001025 rdf:resource="http://purl.obolibrary.org/obo/GAZ_00061709"/>
        <obo:IAO_0000115>A mountain range.</obo:IAO_0000115>
        <oboInOwl:hasOBONamespace>GAZ</oboInOwl:hasOBONamespace>
        <oboInOwl:id>GAZ:00061987</oboInOwl:id>
        <rdfs:label>Sureanu Mountains</rdfs:label>
    </owl:NamedIndividual>
    


    <!-- http://purl.obolibrary.org/obo/GAZ_00061988 -->

    <owl:NamedIndividual rdf:about="http://purl.obolibrary.org/obo/GAZ_00061988">
        <obo:RO_0001025 rdf:resource="http://purl.obolibrary.org/obo/GAZ_00061709"/>
        <obo:IAO_0000115>A depression. Located between Muntii Retezat and Muntii Sebes (N), and Muntii Valcan and Parang (S).</obo:IAO_0000115>
        <oboInOwl:hasOBONamespace>GAZ</oboInOwl:hasOBONamespace>
        <oboInOwl:id>GAZ:00061988</oboInOwl:id>
        <rdfs:label>Depresiunea Petrosani</rdfs:label>
    </owl:NamedIndividual>
    


    <!-- http://purl.obolibrary.org/obo/GAZ_00061989 -->

    <owl:NamedIndividual rdf:about="http://purl.obolibrary.org/obo/GAZ_00061989">
        <obo:RO_0001025 rdf:resource="http://purl.obolibrary.org/obo/GAZ_00061709"/>
        <obo:IAO_0000115>A mountain range.</obo:IAO_0000115>
        <oboInOwl:hasOBONamespace>GAZ</oboInOwl:hasOBONamespace>
        <oboInOwl:id>GAZ:00061989</oboInOwl:id>
        <rdfs:label>Muntii Capatanii</rdfs:label>
    </owl:NamedIndividual>
    


    <!-- http://purl.obolibrary.org/obo/GAZ_00061990 -->

    <owl:NamedIndividual rdf:about="http://purl.obolibrary.org/obo/GAZ_00061990">
        <obo:RO_0001025 rdf:resource="http://purl.obolibrary.org/obo/GAZ_00061709"/>
        <obo:IAO_0000115>A group of mountains in central Romania in the center of the Southern Carpathians, in the North-East of the Parang Mountains group. The main river flowing from the mountain is the Cibin river, which collects most of the other smaller rivers. Between the Cindrel Mountains and the Transylvanian Plateau, the river forms a wide depression the Sibiu Depression in which the main city in the area lies (Sibiu).</obo:IAO_0000115>
        <oboInOwl:hasOBONamespace>GAZ</oboInOwl:hasOBONamespace>
        <oboInOwl:id>GAZ:00061990</oboInOwl:id>
        <rdfs:label>Cindrel Mountains</rdfs:label>
    </owl:NamedIndividual>
    


    <!-- http://purl.obolibrary.org/obo/GAZ_00061991 -->

    <owl:NamedIndividual rdf:about="http://purl.obolibrary.org/obo/GAZ_00061991">
        <obo:RO_0001025 rdf:resource="http://purl.obolibrary.org/obo/GAZ_00061709"/>
        <oboInOwl:hasOBONamespace>GAZ</oboInOwl:hasOBONamespace>
        <oboInOwl:id>GAZ:00061991</oboInOwl:id>
        <rdfs:label>Lotru Mountains</rdfs:label>
    </owl:NamedIndividual>
    


    <!-- http://purl.obolibrary.org/obo/GAZ_00061993 -->

    <owl:NamedIndividual rdf:about="http://purl.obolibrary.org/obo/GAZ_00061993">
        <obo:RO_0001025 rdf:resource="http://purl.obolibrary.org/obo/GAZ_00061709"/>
        <obo:IAO_0000115>One of the highest mountain ridges in Romania and Southern Carpathians.</obo:IAO_0000115>
        <oboInOwl:hasOBONamespace>GAZ</oboInOwl:hasOBONamespace>
        <oboInOwl:id>GAZ:00061993</oboInOwl:id>
        <rdfs:label>Parang Mountains</rdfs:label>
    </owl:NamedIndividual>
    


    <!-- http://purl.obolibrary.org/obo/GAZ_00061994 -->

    <owl:NamedIndividual rdf:about="http://purl.obolibrary.org/obo/GAZ_00061994">
        <obo:RO_0001025 rdf:resource="http://purl.obolibrary.org/obo/GAZ_00061708"/>
        <obo:IAO_0000115>The highest mountains of the Southern Carpathians, in Romania. They are bordered in the north by the Fagaras Depression, through which the Olt river flows, and in the west by the Olt Valley (Valea Oltului). The city Fagsras lies north of the mountains. The most important city in the area is Sibiu.</obo:IAO_0000115>
        <oboInOwl:hasOBONamespace>GAZ</oboInOwl:hasOBONamespace>
        <oboInOwl:id>GAZ:00061994</oboInOwl:id>
        <rdfs:label>Fagaras Mountains</rdfs:label>
    </owl:NamedIndividual>
    


    <!-- http://purl.obolibrary.org/obo/GAZ_00061995 -->

    <owl:NamedIndividual rdf:about="http://purl.obolibrary.org/obo/GAZ_00061995">
        <obo:RO_0001025 rdf:resource="http://purl.obolibrary.org/obo/GAZ_00061708"/>
        <obo:IAO_0000115>A mountain range.</obo:IAO_0000115>
        <oboInOwl:hasOBONamespace>GAZ</oboInOwl:hasOBONamespace>
        <oboInOwl:id>GAZ:00061995</oboInOwl:id>
        <rdfs:label>Cozia Mountains</rdfs:label>
    </owl:NamedIndividual>
    


    <!-- http://purl.obolibrary.org/obo/GAZ_00061996 -->

    <owl:NamedIndividual rdf:about="http://purl.obolibrary.org/obo/GAZ_00061996">
        <obo:RO_0001025 rdf:resource="http://purl.obolibrary.org/obo/GAZ_00061708"/>
        <oboInOwl:hasOBONamespace>GAZ</oboInOwl:hasOBONamespace>
        <oboInOwl:id>GAZ:00061996</oboInOwl:id>
        <rdfs:label>Loviste Depression</rdfs:label>
    </owl:NamedIndividual>
    


    <!-- http://purl.obolibrary.org/obo/GAZ_00061997 -->

    <owl:NamedIndividual rdf:about="http://purl.obolibrary.org/obo/GAZ_00061997">
        <obo:RO_0001025 rdf:resource="http://purl.obolibrary.org/obo/GAZ_00061708"/>
        <obo:IAO_0000115>A mountain range.</obo:IAO_0000115>
        <oboInOwl:hasOBONamespace>GAZ</oboInOwl:hasOBONamespace>
        <oboInOwl:id>GAZ:00061997</oboInOwl:id>
        <rdfs:label>Iezer Mountains</rdfs:label>
    </owl:NamedIndividual>
    


    <!-- http://purl.obolibrary.org/obo/GAZ_00061998 -->

    <owl:NamedIndividual rdf:about="http://purl.obolibrary.org/obo/GAZ_00061998">
        <obo:RO_0001025 rdf:resource="http://purl.obolibrary.org/obo/GAZ_00062003"/>
        <obo:RO_0001025 rdf:resource="http://purl.obolibrary.org/obo/GAZ_00062006"/>
        <obo:IAO_0000115>A glacier cirque lake, situated in the Retezat Mountains, in Romania. It is located south of the main ridge, at the base of Peleaga Peak, and at an altitude of about 2,040 m.</obo:IAO_0000115>
        <oboInOwl:hasOBONamespace>GAZ</oboInOwl:hasOBONamespace>
        <oboInOwl:id>GAZ:00061998</oboInOwl:id>
        <rdfs:label>Bucura Lake</rdfs:label>
    </owl:NamedIndividual>
    


    <!-- http://purl.obolibrary.org/obo/GAZ_00061999 -->

    <owl:NamedIndividual rdf:about="http://purl.obolibrary.org/obo/GAZ_00061999">
        <obo:RO_0001025 rdf:resource="http://purl.obolibrary.org/obo/GAZ_00061710"/>
        <oboInOwl:hasOBONamespace>GAZ</oboInOwl:hasOBONamespace>
        <oboInOwl:id>GAZ:00061999</oboInOwl:id>
        <rdfs:label>Cerna Mountains</rdfs:label>
    </owl:NamedIndividual>
    


    <!-- http://purl.obolibrary.org/obo/GAZ_00062000 -->

    <owl:NamedIndividual rdf:about="http://purl.obolibrary.org/obo/GAZ_00062000">
        <obo:RO_0001025 rdf:resource="http://purl.obolibrary.org/obo/GAZ_00061710"/>
        <oboInOwl:hasOBONamespace>GAZ</oboInOwl:hasOBONamespace>
        <oboInOwl:id>GAZ:00062000</oboInOwl:id>
        <rdfs:label>Godeanu Mountains</rdfs:label>
    </owl:NamedIndividual>
    


    <!-- http://purl.obolibrary.org/obo/GAZ_00062001 -->

    <owl:NamedIndividual rdf:about="http://purl.obolibrary.org/obo/GAZ_00062001">
        <obo:RO_0001025 rdf:resource="http://purl.obolibrary.org/obo/GAZ_00061710"/>
        <obo:IAO_0000115>A mountain range in the southwestern Romania, at the western edge of the Southern Carpathians. They are located between the Bistra Valley (to the north), Timis River (to the east), Godeanu Mountains (to the south) and aaul Mare Valley (to the west).</obo:IAO_0000115>
        <oboInOwl:hasOBONamespace>GAZ</oboInOwl:hasOBONamespace>
        <oboInOwl:id>GAZ:00062001</oboInOwl:id>
        <rdfs:label>Tarcu Mountains</rdfs:label>
    </owl:NamedIndividual>
    


    <!-- http://purl.obolibrary.org/obo/GAZ_00062002 -->

    <owl:NamedIndividual rdf:about="http://purl.obolibrary.org/obo/GAZ_00062002">
        <obo:RO_0001025 rdf:resource="http://purl.obolibrary.org/obo/GAZ_00061710"/>
        <obo:IAO_0000115>A mountain range.</obo:IAO_0000115>
        <oboInOwl:hasOBONamespace>GAZ</oboInOwl:hasOBONamespace>
        <oboInOwl:id>GAZ:00062002</oboInOwl:id>
        <rdfs:label>Mehedinti Mountains</rdfs:label>
    </owl:NamedIndividual>
    


    <!-- http://purl.obolibrary.org/obo/GAZ_00062003 -->

    <owl:NamedIndividual rdf:about="http://purl.obolibrary.org/obo/GAZ_00062003">
        <obo:RO_0001025 rdf:resource="http://purl.obolibrary.org/obo/GAZ_00061710"/>
        <obo:IAO_0000115>Mountains that are part of the Southern Carpathians.</obo:IAO_0000115>
        <oboInOwl:hasOBONamespace>GAZ</oboInOwl:hasOBONamespace>
        <oboInOwl:id>GAZ:00062003</oboInOwl:id>
        <rdfs:label>Retezat Mountains</rdfs:label>
    </owl:NamedIndividual>
    


    <!-- http://purl.obolibrary.org/obo/GAZ_00062004 -->

    <owl:NamedIndividual rdf:about="http://purl.obolibrary.org/obo/GAZ_00062004">
        <obo:RO_0001025 rdf:resource="http://purl.obolibrary.org/obo/GAZ_00061710"/>
        <obo:IAO_0000115>A chain of mountains in the southern Carpathians in Romania.</obo:IAO_0000115>
        <oboInOwl:hasOBONamespace>GAZ</oboInOwl:hasOBONamespace>
        <oboInOwl:id>GAZ:00062004</oboInOwl:id>
        <rdfs:label>Valcan Mountains</rdfs:label>
    </owl:NamedIndividual>
    


    <!-- http://purl.obolibrary.org/obo/GAZ_00062006 -->

    <owl:NamedIndividual rdf:about="http://purl.obolibrary.org/obo/GAZ_00062006">
        <obo:RO_0001025 rdf:resource="http://purl.obolibrary.org/obo/GAZ_00062003"/>
        <obo:IAO_0000115>A national park located in Hunedoara county, Romania, was founded in 1935 and has an area of 380 km2.</obo:IAO_0000115>
        <oboInOwl:hasOBONamespace>GAZ</oboInOwl:hasOBONamespace>
        <oboInOwl:id>GAZ:00062006</oboInOwl:id>
        <rdfs:label>Parcul National Retezat</rdfs:label>
    </owl:NamedIndividual>
    


    <!-- http://purl.obolibrary.org/obo/GAZ_00062008 -->

    <owl:NamedIndividual rdf:about="http://purl.obolibrary.org/obo/GAZ_00062008">
        <obo:RO_0001025 rdf:resource="http://purl.obolibrary.org/obo/GAZ_00061705"/>
        <oboInOwl:hasOBONamespace>GAZ</oboInOwl:hasOBONamespace>
        <oboInOwl:id>GAZ:00062008</oboInOwl:id>
        <rdfs:label>Cris Mountains</rdfs:label>
    </owl:NamedIndividual>
    


    <!-- http://purl.obolibrary.org/obo/GAZ_00062009 -->

    <owl:NamedIndividual rdf:about="http://purl.obolibrary.org/obo/GAZ_00062009">
        <obo:RO_0001025 rdf:resource="http://purl.obolibrary.org/obo/GAZ_00062010"/>
        <oboInOwl:hasOBONamespace>GAZ</oboInOwl:hasOBONamespace>
        <oboInOwl:id>GAZ:00062009</oboInOwl:id>
        <rdfs:label>Vad Depression</rdfs:label>
    </owl:NamedIndividual>
    


    <!-- http://purl.obolibrary.org/obo/GAZ_00062010 -->

    <owl:NamedIndividual rdf:about="http://purl.obolibrary.org/obo/GAZ_00062010">
        <obo:RO_0001025 rdf:resource="http://purl.obolibrary.org/obo/GAZ_00062008"/>
        <oboInOwl:hasOBONamespace>GAZ</oboInOwl:hasOBONamespace>
        <oboInOwl:id>GAZ:00062010</oboInOwl:id>
        <rdfs:label>Cris Hills</rdfs:label>
    </owl:NamedIndividual>
    


    <!-- http://purl.obolibrary.org/obo/GAZ_00062011 -->

    <owl:NamedIndividual rdf:about="http://purl.obolibrary.org/obo/GAZ_00062011">
        <obo:RO_0001025 rdf:resource="http://purl.obolibrary.org/obo/GAZ_00062008"/>
        <obo:IAO_0000115>The northwestern part of the Apuseni Mountains of the Carpathian Mountain range, located between the Vad-Borod Depression and Beius Depression. The Dealurile Vestice (Vestice Hills) are located to the west of these mountains and the Vladeasa Mountains are to their east.</obo:IAO_0000115>
        <oboInOwl:hasOBONamespace>GAZ</oboInOwl:hasOBONamespace>
        <oboInOwl:id>GAZ:00062011</oboInOwl:id>
        <rdfs:label>Padurea Craiului</rdfs:label>
    </owl:NamedIndividual>
    


    <!-- http://purl.obolibrary.org/obo/GAZ_00062012 -->

    <owl:NamedIndividual rdf:about="http://purl.obolibrary.org/obo/GAZ_00062012">
        <obo:RO_0001025 rdf:resource="http://purl.obolibrary.org/obo/GAZ_00062010"/>
        <oboInOwl:hasOBONamespace>GAZ</oboInOwl:hasOBONamespace>
        <oboInOwl:id>GAZ:00062012</oboInOwl:id>
        <rdfs:label>Beius Depression</rdfs:label>
    </owl:NamedIndividual>
    


    <!-- http://purl.obolibrary.org/obo/GAZ_00062013 -->

    <owl:NamedIndividual rdf:about="http://purl.obolibrary.org/obo/GAZ_00062013">
        <obo:RO_0001025 rdf:resource="http://purl.obolibrary.org/obo/GAZ_00062008"/>
        <oboInOwl:hasOBONamespace>GAZ</oboInOwl:hasOBONamespace>
        <oboInOwl:id>GAZ:00062013</oboInOwl:id>
        <rdfs:label>Codru-Moma Mountains</rdfs:label>
    </owl:NamedIndividual>
    


    <!-- http://purl.obolibrary.org/obo/GAZ_00062014 -->

    <owl:NamedIndividual rdf:about="http://purl.obolibrary.org/obo/GAZ_00062014">
        <obo:RO_0001025 rdf:resource="http://purl.obolibrary.org/obo/GAZ_00061705"/>
        <oboInOwl:hasOBONamespace>GAZ</oboInOwl:hasOBONamespace>
        <oboInOwl:id>GAZ:00062014</oboInOwl:id>
        <rdfs:label>Ses-Meses Mountains</rdfs:label>
    </owl:NamedIndividual>
    


    <!-- http://purl.obolibrary.org/obo/GAZ_00062015 -->

    <owl:NamedIndividual rdf:about="http://purl.obolibrary.org/obo/GAZ_00062015">
        <obo:RO_0001025 rdf:resource="http://purl.obolibrary.org/obo/GAZ_00062014"/>
        <oboInOwl:hasOBONamespace>GAZ</oboInOwl:hasOBONamespace>
        <oboInOwl:id>GAZ:00062015</oboInOwl:id>
        <rdfs:label>Meses Mountains</rdfs:label>
    </owl:NamedIndividual>
    


    <!-- http://purl.obolibrary.org/obo/GAZ_00062016 -->

    <owl:NamedIndividual rdf:about="http://purl.obolibrary.org/obo/GAZ_00062016">
        <obo:RO_0001025 rdf:resource="http://purl.obolibrary.org/obo/GAZ_00062014"/>
        <oboInOwl:hasOBONamespace>GAZ</oboInOwl:hasOBONamespace>
        <oboInOwl:id>GAZ:00062016</oboInOwl:id>
        <rdfs:label>Ses Mountain</rdfs:label>
    </owl:NamedIndividual>
    


    <!-- http://purl.obolibrary.org/obo/GAZ_00062017 -->

    <owl:NamedIndividual rdf:about="http://purl.obolibrary.org/obo/GAZ_00062017">
        <obo:RO_0001025 rdf:resource="http://purl.obolibrary.org/obo/GAZ_00062014"/>
        <oboInOwl:hasOBONamespace>GAZ</oboInOwl:hasOBONamespace>
        <oboInOwl:id>GAZ:00062017</oboInOwl:id>
        <rdfs:label>Simleu Mountains</rdfs:label>
    </owl:NamedIndividual>
    


    <!-- http://purl.obolibrary.org/obo/GAZ_00062018 -->

    <owl:NamedIndividual rdf:about="http://purl.obolibrary.org/obo/GAZ_00062018">
        <obo:RO_0001025 rdf:resource="http://purl.obolibrary.org/obo/GAZ_00062014"/>
        <oboInOwl:hasOBONamespace>GAZ</oboInOwl:hasOBONamespace>
        <oboInOwl:id>GAZ:00062018</oboInOwl:id>
        <rdfs:label>Simleu Depression</rdfs:label>
    </owl:NamedIndividual>
    


    <!-- http://purl.obolibrary.org/obo/GAZ_00062019 -->

    <owl:NamedIndividual rdf:about="http://purl.obolibrary.org/obo/GAZ_00062019">
        <obo:RO_0001025 rdf:resource="http://purl.obolibrary.org/obo/GAZ_00061705"/>
        <obo:IAO_0000115>A massif located in Romania, in the Romanian Western Carpathians mountain range. The massif has a length of 25 km from the northwest to the southeast and a width of 14 km.</obo:IAO_0000115>
        <oboInOwl:hasOBONamespace>GAZ</oboInOwl:hasOBONamespace>
        <oboInOwl:id>GAZ:00062019</oboInOwl:id>
        <rdfs:label>Bihor Massif</rdfs:label>
    </owl:NamedIndividual>
    


    <!-- http://purl.obolibrary.org/obo/GAZ_00062020 -->

    <owl:NamedIndividual rdf:about="http://purl.obolibrary.org/obo/GAZ_00062020">
        <obo:RO_0001025 rdf:resource="http://purl.obolibrary.org/obo/GAZ_00062019"/>
        <obo:IAO_0000115>A mountain range.</obo:IAO_0000115>
        <oboInOwl:hasOBONamespace>GAZ</oboInOwl:hasOBONamespace>
        <oboInOwl:id>GAZ:00062020</oboInOwl:id>
        <rdfs:label>Bihor Mountains</rdfs:label>
    </owl:NamedIndividual>
    


    <!-- http://purl.obolibrary.org/obo/GAZ_00062021 -->

    <owl:NamedIndividual rdf:about="http://purl.obolibrary.org/obo/GAZ_00062021">
        <obo:RO_0001025 rdf:resource="http://purl.obolibrary.org/obo/GAZ_00062019"/>
        <obo:IAO_0000115>A mountain massif.</obo:IAO_0000115>
        <oboInOwl:hasOBONamespace>GAZ</oboInOwl:hasOBONamespace>
        <oboInOwl:id>GAZ:00062021</oboInOwl:id>
        <rdfs:label>Muntele Mare</rdfs:label>
    </owl:NamedIndividual>
    


    <!-- http://purl.obolibrary.org/obo/GAZ_00062022 -->

    <owl:NamedIndividual rdf:about="http://purl.obolibrary.org/obo/GAZ_00062022">
        <obo:RO_0001025 rdf:resource="http://purl.obolibrary.org/obo/GAZ_00062019"/>
        <obo:IAO_0000115>A mountain range.</obo:IAO_0000115>
        <oboInOwl:hasOBONamespace>GAZ</oboInOwl:hasOBONamespace>
        <oboInOwl:id>GAZ:00062022</oboInOwl:id>
        <rdfs:label>Gilau Mountains</rdfs:label>
    </owl:NamedIndividual>
    


    <!-- http://purl.obolibrary.org/obo/GAZ_00062023 -->

    <owl:NamedIndividual rdf:about="http://purl.obolibrary.org/obo/GAZ_00062023">
        <obo:RO_0001025 rdf:resource="http://purl.obolibrary.org/obo/GAZ_00061705"/>
        <oboInOwl:hasOBONamespace>GAZ</oboInOwl:hasOBONamespace>
        <oboInOwl:id>GAZ:00062023</oboInOwl:id>
        <rdfs:label>Mures Mountains</rdfs:label>
    </owl:NamedIndividual>
    


    <!-- http://purl.obolibrary.org/obo/GAZ_00062024 -->

    <owl:NamedIndividual rdf:about="http://purl.obolibrary.org/obo/GAZ_00062024">
        <obo:RO_0001025 rdf:resource="http://purl.obolibrary.org/obo/GAZ_00062023"/>
        <obo:IAO_0000115>A mountain range.</obo:IAO_0000115>
        <oboInOwl:hasOBONamespace>GAZ</oboInOwl:hasOBONamespace>
        <oboInOwl:id>GAZ:00062024</oboInOwl:id>
        <rdfs:label>Metalliferous Mountains</rdfs:label>
    </owl:NamedIndividual>
    


    <!-- http://purl.obolibrary.org/obo/GAZ_00062025 -->

    <owl:NamedIndividual rdf:about="http://purl.obolibrary.org/obo/GAZ_00062025">
        <obo:RO_0001025 rdf:resource="http://purl.obolibrary.org/obo/GAZ_00062024"/>
        <obo:IAO_0000115>A mountain range located in the Apuseni mountain range of the Western Carpathian Mountains, in Romania. They are crossed by Aries River valley.</obo:IAO_0000115>
        <oboInOwl:hasOBONamespace>GAZ</oboInOwl:hasOBONamespace>
        <oboInOwl:id>GAZ:00062025</oboInOwl:id>
        <rdfs:label>Trascau Mountains</rdfs:label>
    </owl:NamedIndividual>
    


    <!-- http://purl.obolibrary.org/obo/GAZ_00062026 -->

    <owl:NamedIndividual rdf:about="http://purl.obolibrary.org/obo/GAZ_00062026">
        <obo:RO_0001025 rdf:resource="http://purl.obolibrary.org/obo/GAZ_00062023"/>
        <oboInOwl:hasOBONamespace>GAZ</oboInOwl:hasOBONamespace>
        <oboInOwl:id>GAZ:00062026</oboInOwl:id>
        <rdfs:label>Zarand Mountains</rdfs:label>
    </owl:NamedIndividual>
    


    <!-- http://purl.obolibrary.org/obo/GAZ_00062027 -->

    <owl:NamedIndividual rdf:about="http://purl.obolibrary.org/obo/GAZ_00062027">
        <obo:RO_0001025 rdf:resource="http://purl.obolibrary.org/obo/GAZ_00061700"/>
        <obo:IAO_0000115>A mountain range.Situated roughly south of the river Mures, northeast of the river Timis and west of the river Strei.</obo:IAO_0000115>
        <oboInOwl:hasOBONamespace>GAZ</oboInOwl:hasOBONamespace>
        <oboInOwl:id>GAZ:00062027</oboInOwl:id>
        <rdfs:label>Poiana Rusca Mountains</rdfs:label>
    </owl:NamedIndividual>
    


    <!-- http://purl.obolibrary.org/obo/GAZ_00062028 -->

    <owl:NamedIndividual rdf:about="http://purl.obolibrary.org/obo/GAZ_00062028">
        <obo:RO_0001025 rdf:resource="http://purl.obolibrary.org/obo/GAZ_00062027"/>
        <oboInOwl:hasOBONamespace>GAZ</oboInOwl:hasOBONamespace>
        <oboInOwl:id>GAZ:00062028</oboInOwl:id>
        <rdfs:label>Lipova Plateau</rdfs:label>
    </owl:NamedIndividual>
    


    <!-- http://purl.obolibrary.org/obo/GAZ_00062029 -->

    <owl:NamedIndividual rdf:about="http://purl.obolibrary.org/obo/GAZ_00062029">
        <obo:RO_0001025 rdf:resource="http://purl.obolibrary.org/obo/GAZ_00062027"/>
        <oboInOwl:hasOBONamespace>GAZ</oboInOwl:hasOBONamespace>
        <oboInOwl:id>GAZ:00062029</oboInOwl:id>
        <rdfs:label>Orastie Groove</rdfs:label>
    </owl:NamedIndividual>
    


    <!-- http://purl.obolibrary.org/obo/GAZ_00062031 -->

    <owl:NamedIndividual rdf:about="http://purl.obolibrary.org/obo/GAZ_00062031">
        <obo:RO_0001025 rdf:resource="http://purl.obolibrary.org/obo/GAZ_00062027"/>
        <oboInOwl:hasOBONamespace>GAZ</oboInOwl:hasOBONamespace>
        <oboInOwl:id>GAZ:00062031</oboInOwl:id>
        <rdfs:label>Bega-Timis Groove</rdfs:label>
    </owl:NamedIndividual>
    


    <!-- http://purl.obolibrary.org/obo/GAZ_00062032 -->

    <owl:NamedIndividual rdf:about="http://purl.obolibrary.org/obo/GAZ_00062032">
        <obo:RO_0001025 rdf:resource="http://purl.obolibrary.org/obo/GAZ_00061706"/>
        <oboInOwl:hasOBONamespace>GAZ</oboInOwl:hasOBONamespace>
        <oboInOwl:id>GAZ:00062032</oboInOwl:id>
        <rdfs:label>Almaj Mountains</rdfs:label>
    </owl:NamedIndividual>
    


    <!-- http://purl.obolibrary.org/obo/GAZ_00062033 -->

    <owl:NamedIndividual rdf:about="http://purl.obolibrary.org/obo/GAZ_00062033">
        <obo:RO_0001025 rdf:resource="http://purl.obolibrary.org/obo/GAZ_00061706"/>
        <obo:IAO_0000115>A mountain pass in South-Western Romania (mostly in Caras-Severin County), dividing the Southern Carpathians and Banat mountain ranges, both part of the Carpathians. The pass follows the paths of the rivers Timis (which flows northward) and Cerna (which flows southward). To the west lie the Almaj and Semenic Mountains and to the east Mehedinti, Cerna, Tarcului and Poiana Rusca Mountains. The town of Caransebes lies in the Timis-Cerna Gap and Orsova lies on the Danube at the gap&apos;s southern end.</obo:IAO_0000115>
        <oboInOwl:hasOBONamespace>GAZ</oboInOwl:hasOBONamespace>
        <oboInOwl:id>GAZ:00062033</oboInOwl:id>
        <rdfs:label>Timis-Cerna Groove</rdfs:label>
    </owl:NamedIndividual>
    


    <!-- http://purl.obolibrary.org/obo/GAZ_00062034 -->

    <owl:NamedIndividual rdf:about="http://purl.obolibrary.org/obo/GAZ_00062034">
        <obo:RO_0001025 rdf:resource="http://purl.obolibrary.org/obo/GAZ_00061706"/>
        <oboInOwl:hasOBONamespace>GAZ</oboInOwl:hasOBONamespace>
        <oboInOwl:id>GAZ:00062034</oboInOwl:id>
        <rdfs:label>Caras Hills</rdfs:label>
    </owl:NamedIndividual>
    


    <!-- http://purl.obolibrary.org/obo/GAZ_00062035 -->

    <owl:NamedIndividual rdf:about="http://purl.obolibrary.org/obo/GAZ_00062035">
        <obo:RO_0001025 rdf:resource="http://purl.obolibrary.org/obo/GAZ_00062033"/>
        <oboInOwl:hasOBONamespace>GAZ</oboInOwl:hasOBONamespace>
        <oboInOwl:id>GAZ:00062035</oboInOwl:id>
        <rdfs:label>Almaj Depression</rdfs:label>
    </owl:NamedIndividual>
    


    <!-- http://purl.obolibrary.org/obo/GAZ_00062036 -->

    <owl:NamedIndividual rdf:about="http://purl.obolibrary.org/obo/GAZ_00062036">
        <obo:RO_0001025 rdf:resource="http://purl.obolibrary.org/obo/GAZ_00061706"/>
        <oboInOwl:hasOBONamespace>GAZ</oboInOwl:hasOBONamespace>
        <oboInOwl:id>GAZ:00062036</oboInOwl:id>
        <rdfs:label>Banat Mountains</rdfs:label>
    </owl:NamedIndividual>
    


    <!-- http://purl.obolibrary.org/obo/GAZ_00062037 -->

    <owl:NamedIndividual rdf:about="http://purl.obolibrary.org/obo/GAZ_00062037">
        <obo:RO_0001025 rdf:resource="http://purl.obolibrary.org/obo/GAZ_00062036"/>
        <oboInOwl:hasOBONamespace>GAZ</oboInOwl:hasOBONamespace>
        <oboInOwl:id>GAZ:00062037</oboInOwl:id>
        <rdfs:label>Locva Mountains</rdfs:label>
    </owl:NamedIndividual>
    


    <!-- http://purl.obolibrary.org/obo/GAZ_00062038 -->

    <owl:NamedIndividual rdf:about="http://purl.obolibrary.org/obo/GAZ_00062038">
        <obo:RO_0001025 rdf:resource="http://purl.obolibrary.org/obo/GAZ_00062036"/>
        <obo:IAO_0000115>A mountain range.</obo:IAO_0000115>
        <oboInOwl:hasOBONamespace>GAZ</oboInOwl:hasOBONamespace>
        <oboInOwl:id>GAZ:00062038</oboInOwl:id>
        <rdfs:label>Anina Mountains</rdfs:label>
    </owl:NamedIndividual>
    


    <!-- http://purl.obolibrary.org/obo/GAZ_00062039 -->

    <owl:NamedIndividual rdf:about="http://purl.obolibrary.org/obo/GAZ_00062039">
        <obo:RO_0001025 rdf:resource="http://purl.obolibrary.org/obo/GAZ_00062036"/>
        <obo:IAO_0000115>A mountain range.</obo:IAO_0000115>
        <oboInOwl:hasOBONamespace>GAZ</oboInOwl:hasOBONamespace>
        <oboInOwl:id>GAZ:00062039</oboInOwl:id>
        <rdfs:label>Dognecea Mountains</rdfs:label>
    </owl:NamedIndividual>
    


    <!-- http://purl.obolibrary.org/obo/GAZ_00062040 -->

    <owl:NamedIndividual rdf:about="http://purl.obolibrary.org/obo/GAZ_00062040">
        <obo:RO_0001025 rdf:resource="http://purl.obolibrary.org/obo/GAZ_00061701"/>
        <oboInOwl:hasOBONamespace>GAZ</oboInOwl:hasOBONamespace>
        <oboInOwl:id>GAZ:00062040</oboInOwl:id>
        <rdfs:label>Beljanica Mountain</rdfs:label>
    </owl:NamedIndividual>
    


    <!-- http://purl.obolibrary.org/obo/GAZ_00062041 -->

    <owl:NamedIndividual rdf:about="http://purl.obolibrary.org/obo/GAZ_00062041">
        <obo:RO_0001025 rdf:resource="http://purl.obolibrary.org/obo/GAZ_00061701"/>
        <oboInOwl:hasOBONamespace>GAZ</oboInOwl:hasOBONamespace>
        <oboInOwl:id>GAZ:00062041</oboInOwl:id>
        <rdfs:label>Miroc Mountain</rdfs:label>
    </owl:NamedIndividual>
    


    <!-- http://purl.obolibrary.org/obo/GAZ_00062042 -->

    <owl:NamedIndividual rdf:about="http://purl.obolibrary.org/obo/GAZ_00062042">
        <obo:RO_0001025 rdf:resource="http://purl.obolibrary.org/obo/GAZ_00061701"/>
        <oboInOwl:hasOBONamespace>GAZ</oboInOwl:hasOBONamespace>
        <oboInOwl:id>GAZ:00062042</oboInOwl:id>
        <rdfs:label>Ozren and Devica</rdfs:label>
    </owl:NamedIndividual>
    


    <!-- http://purl.obolibrary.org/obo/GAZ_00062043 -->

    <owl:NamedIndividual rdf:about="http://purl.obolibrary.org/obo/GAZ_00062043">
        <obo:RO_0001025 rdf:resource="http://purl.obolibrary.org/obo/GAZ_00061701"/>
        <oboInOwl:hasOBONamespace>GAZ</oboInOwl:hasOBONamespace>
        <oboInOwl:id>GAZ:00062043</oboInOwl:id>
        <rdfs:label>Rtanj Mountain</rdfs:label>
    </owl:NamedIndividual>
    


    <!-- http://purl.obolibrary.org/obo/GAZ_00062044 -->

    <owl:NamedIndividual rdf:about="http://purl.obolibrary.org/obo/GAZ_00062044">
        <obo:RO_0001025 rdf:resource="http://purl.obolibrary.org/obo/GAZ_00061701"/>
        <oboInOwl:hasOBONamespace>GAZ</oboInOwl:hasOBONamespace>
        <oboInOwl:id>GAZ:00062044</oboInOwl:id>
        <rdfs:label>Homolj Mountains</rdfs:label>
    </owl:NamedIndividual>
    


    <!-- http://purl.obolibrary.org/obo/GAZ_00062045 -->

    <owl:NamedIndividual rdf:about="http://purl.obolibrary.org/obo/GAZ_00062045">
        <obo:RO_0001025 rdf:resource="http://purl.obolibrary.org/obo/GAZ_00061701"/>
        <oboInOwl:hasOBONamespace>GAZ</oboInOwl:hasOBONamespace>
        <oboInOwl:id>GAZ:00062045</oboInOwl:id>
        <rdfs:label>Kucaj Mountains</rdfs:label>
    </owl:NamedIndividual>
    


    <!-- http://purl.obolibrary.org/obo/GAZ_00062046 -->

    <owl:NamedIndividual rdf:about="http://purl.obolibrary.org/obo/GAZ_00062046">
        <obo:RO_0001025 rdf:resource="http://purl.obolibrary.org/obo/GAZ_00061701"/>
        <oboInOwl:hasOBONamespace>GAZ</oboInOwl:hasOBONamespace>
        <oboInOwl:id>GAZ:00062046</oboInOwl:id>
        <rdfs:label>Deli Jovan</rdfs:label>
    </owl:NamedIndividual>
    


    <!-- http://purl.obolibrary.org/obo/GAZ_00062047 -->

    <owl:NamedIndividual rdf:about="http://purl.obolibrary.org/obo/GAZ_00062047">
        <obo:RO_0001025 rdf:resource="http://purl.obolibrary.org/obo/GAZ_00061701"/>
        <oboInOwl:hasOBONamespace>GAZ</oboInOwl:hasOBONamespace>
        <oboInOwl:id>GAZ:00062047</oboInOwl:id>
        <rdfs:label>Great and Little Krs</rdfs:label>
    </owl:NamedIndividual>
    


    <!-- http://purl.obolibrary.org/obo/GAZ_00062048 -->

    <owl:NamedIndividual rdf:about="http://purl.obolibrary.org/obo/GAZ_00062048">
        <obo:RO_0001025 rdf:resource="http://purl.obolibrary.org/obo/GAZ_00061699"/>
        <oboInOwl:hasOBONamespace>GAZ</oboInOwl:hasOBONamespace>
        <oboInOwl:id>GAZ:00062048</oboInOwl:id>
        <rdfs:label>Tarnava Plateau</rdfs:label>
    </owl:NamedIndividual>
    


    <!-- http://purl.obolibrary.org/obo/GAZ_00062049 -->

    <owl:NamedIndividual rdf:about="http://purl.obolibrary.org/obo/GAZ_00062049">
        <obo:RO_0001025 rdf:resource="http://purl.obolibrary.org/obo/GAZ_00062048"/>
        <oboInOwl:hasOBONamespace>GAZ</oboInOwl:hasOBONamespace>
        <oboInOwl:id>GAZ:00062049</oboInOwl:id>
        <rdfs:label>Secase Plateau</rdfs:label>
    </owl:NamedIndividual>
    


    <!-- http://purl.obolibrary.org/obo/GAZ_00062050 -->

    <owl:NamedIndividual rdf:about="http://purl.obolibrary.org/obo/GAZ_00062050">
        <obo:RO_0001025 rdf:resource="http://purl.obolibrary.org/obo/GAZ_00062048"/>
        <oboInOwl:hasOBONamespace>GAZ</oboInOwl:hasOBONamespace>
        <oboInOwl:id>GAZ:00062050</oboInOwl:id>
        <rdfs:label>Hartibaci Plateau</rdfs:label>
    </owl:NamedIndividual>
    


    <!-- http://purl.obolibrary.org/obo/GAZ_00062051 -->

    <owl:NamedIndividual rdf:about="http://purl.obolibrary.org/obo/GAZ_00062051">
        <obo:RO_0001025 rdf:resource="http://purl.obolibrary.org/obo/GAZ_00061699"/>
        <oboInOwl:hasOBONamespace>GAZ</oboInOwl:hasOBONamespace>
        <oboInOwl:id>GAZ:00062051</oboInOwl:id>
        <rdfs:label>Somes Plateau</rdfs:label>
    </owl:NamedIndividual>
    


    <!-- http://purl.obolibrary.org/obo/GAZ_00062052 -->

    <owl:NamedIndividual rdf:about="http://purl.obolibrary.org/obo/GAZ_00062052">
        <obo:RO_0001025 rdf:resource="http://purl.obolibrary.org/obo/GAZ_00061699"/>
        <oboInOwl:hasOBONamespace>GAZ</oboInOwl:hasOBONamespace>
        <oboInOwl:id>GAZ:00062052</oboInOwl:id>
        <rdfs:label>Transylvanian Plain</rdfs:label>
    </owl:NamedIndividual>
    


    <!-- http://purl.obolibrary.org/obo/GAZ_00062479 -->

    <owl:NamedIndividual rdf:about="http://purl.obolibrary.org/obo/GAZ_00062479">
        <obo:RO_0001025 rdf:resource="http://purl.obolibrary.org/obo/GAZ_00062480"/>
        <obo:IAO_0000115>A lake located in the Vihorlat Mountains in the east of Slovakia.</obo:IAO_0000115>
        <oboInOwl:hasOBONamespace>GAZ</oboInOwl:hasOBONamespace>
        <oboInOwl:id>GAZ:00062479</oboInOwl:id>
        <rdfs:label>Morske oko</rdfs:label>
    </owl:NamedIndividual>
    


    <!-- http://purl.obolibrary.org/obo/GAZ_00062480 -->

    <owl:NamedIndividual rdf:about="http://purl.obolibrary.org/obo/GAZ_00062480">
        <obo:RO_0001025 rdf:resource="http://purl.obolibrary.org/obo/GAZ_00061955"/>
        <obo:IAO_0000115>A protected area.</obo:IAO_0000115>
        <oboInOwl:hasOBONamespace>GAZ</oboInOwl:hasOBONamespace>
        <oboInOwl:id>GAZ:00062480</oboInOwl:id>
        <rdfs:label>National Nature Reserve Morske oko</rdfs:label>
    </owl:NamedIndividual>
    


    <!-- http://purl.obolibrary.org/obo/GAZ_00062483 -->

    <owl:NamedIndividual rdf:about="http://purl.obolibrary.org/obo/GAZ_00062483">
        <obo:IAO_0000115>A lake located in the Bohinj municipality in the north-west of the country, and is inside Triglav National Park. It lies on the Sava Bohinjka river. Lake Bohinj is 4.2 km long and 1 km at its maximum width. It is a glacial lake dammed by a moraine.</obo:IAO_0000115>
        <oboInOwl:hasOBONamespace>GAZ</oboInOwl:hasOBONamespace>
        <oboInOwl:id>GAZ:00062483</oboInOwl:id>
        <rdfs:label>Lake Bohinj</rdfs:label>
    </owl:NamedIndividual>
    


    <!-- http://purl.obolibrary.org/obo/GAZ_00062744 -->

    <owl:NamedIndividual rdf:about="http://purl.obolibrary.org/obo/GAZ_00062744">
        <obo:IAO_0000115>An artificial lake created southwest of the Knic, as a water reservoir.</obo:IAO_0000115>
        <oboInOwl:hasOBONamespace>GAZ</oboInOwl:hasOBONamespace>
        <oboInOwl:id>GAZ:00062744</oboInOwl:id>
        <rdfs:label>Gruza Reservoir</rdfs:label>
    </owl:NamedIndividual>
    


    <!-- http://purl.obolibrary.org/obo/GAZ_00062759 -->

    <owl:NamedIndividual rdf:about="http://purl.obolibrary.org/obo/GAZ_00062759">
        <obo:RO_0001025 rdf:resource="http://purl.obolibrary.org/obo/GAZ_00043912"/>
        <obo:IAO_0000115>A canal turned lake on the Great War Island, within proper of the City of Belgrade, the capital of Serbia.</obo:IAO_0000115>
        <oboInOwl:hasOBONamespace>GAZ</oboInOwl:hasOBONamespace>
        <oboInOwl:id>GAZ:00062759</oboInOwl:id>
        <rdfs:label>Veliki Galijas</rdfs:label>
    </owl:NamedIndividual>
    


    <!-- http://purl.obolibrary.org/obo/GAZ_00062762 -->

    <owl:NamedIndividual rdf:about="http://purl.obolibrary.org/obo/GAZ_00062762">
        <obo:RO_0001025 rdf:resource="http://purl.obolibrary.org/obo/GAZ_00062763"/>
        <obo:IAO_0000115>A semi-artificial lake in Southeast Serbia. It was created in 1947 to 1951, when the peat bog called Vlasinsko blato was closed by a dam and submerged by waters of incoming rivers, chiefly Vlasina.</obo:IAO_0000115>
        <oboInOwl:hasOBONamespace>GAZ</oboInOwl:hasOBONamespace>
        <oboInOwl:id>GAZ:00062762</oboInOwl:id>
        <rdfs:label>Vlasina Lake</rdfs:label>
    </owl:NamedIndividual>
    


    <!-- http://purl.obolibrary.org/obo/GAZ_00062763 -->

    <owl:NamedIndividual rdf:about="http://purl.obolibrary.org/obo/GAZ_00062763">
        <obo:IAO_0000115>A mountaineous region of southeastern Serbia. It is a border area to Bulgaria, a region of the Rhodopian Serbia.</obo:IAO_0000115>
        <oboInOwl:hasOBONamespace>GAZ</oboInOwl:hasOBONamespace>
        <oboInOwl:id>GAZ:00062763</oboInOwl:id>
        <rdfs:label>Vlasina</rdfs:label>
    </owl:NamedIndividual>
    


    <!-- http://purl.obolibrary.org/obo/GAZ_00062765 -->

    <owl:NamedIndividual rdf:about="http://purl.obolibrary.org/obo/GAZ_00062765">
        <obo:RO_0001025 rdf:resource="http://purl.obolibrary.org/obo/GAZ_00062762"/>
        <obo:IAO_0000115>An island in the Vlasina Lake.</obo:IAO_0000115>
        <oboInOwl:hasOBONamespace>GAZ</oboInOwl:hasOBONamespace>
        <oboInOwl:id>GAZ:00062765</oboInOwl:id>
        <rdfs:label>Dugi del Island</rdfs:label>
    </owl:NamedIndividual>
    


    <!-- http://purl.obolibrary.org/obo/GAZ_00062766 -->

    <owl:NamedIndividual rdf:about="http://purl.obolibrary.org/obo/GAZ_00062766">
        <obo:RO_0001025 rdf:resource="http://purl.obolibrary.org/obo/GAZ_00062762"/>
        <obo:IAO_0000115>An island in the Vlasina Lake.</obo:IAO_0000115>
        <oboInOwl:hasOBONamespace>GAZ</oboInOwl:hasOBONamespace>
        <oboInOwl:id>GAZ:00062766</oboInOwl:id>
        <rdfs:label>Stratorija Island</rdfs:label>
    </owl:NamedIndividual>
    


    <!-- http://purl.obolibrary.org/obo/GAZ_00062767 -->

    <owl:NamedIndividual rdf:about="http://purl.obolibrary.org/obo/GAZ_00062767">
        <obo:RO_0001025 rdf:resource="http://purl.obolibrary.org/obo/GAZ_00062762"/>
        <obo:IAO_0000115>A floating island, made of peat, in Vlasina Lake. Often anchored to the shore.</obo:IAO_0000115>
        <oboInOwl:hasOBONamespace>GAZ</oboInOwl:hasOBONamespace>
        <oboInOwl:id>GAZ:00062767</oboInOwl:id>
        <rdfs:label>Moby Dick</rdfs:label>
    </owl:NamedIndividual>
    


    <!-- http://purl.obolibrary.org/obo/GAZ_00062771 -->

    <owl:NamedIndividual rdf:about="http://purl.obolibrary.org/obo/GAZ_00062771">
        <obo:IAO_0000115>A lake formed from a dammed arm of the Sava River, adjacent to Ada Ciganlija Island.</obo:IAO_0000115>
        <oboInOwl:hasOBONamespace>GAZ</oboInOwl:hasOBONamespace>
        <oboInOwl:id>GAZ:00062771</oboInOwl:id>
        <rdfs:label>Sava Lake</rdfs:label>
    </owl:NamedIndividual>
    


    <!-- http://purl.obolibrary.org/obo/GAZ_00062773 -->

    <owl:NamedIndividual rdf:about="http://purl.obolibrary.org/obo/GAZ_00062773">
        <obo:IAO_0000115>An artificial lake that is a fish pond, where the Jegricka River flows into the marshes of Zabalj.</obo:IAO_0000115>
        <oboInOwl:hasOBONamespace>GAZ</oboInOwl:hasOBONamespace>
        <oboInOwl:id>GAZ:00062773</oboInOwl:id>
        <rdfs:label>Jegricka Fish Pond</rdfs:label>
    </owl:NamedIndividual>
    


    <!-- http://purl.obolibrary.org/obo/GAZ_00062780 -->

    <owl:NamedIndividual rdf:about="http://purl.obolibrary.org/obo/GAZ_00062780">
        <obo:IAO_0000115>A large swamp-forest area and natural reserve stretching along the Sava River in Southern Syrmia (Serbia), some 40 km west of Belgrade. The pond is an oxbow lake, a remnant of the meanders of the old Sava river, whose main stream nowadays flows more southward. Due to its shape, swampy bed of the pond, situated between the villages of Obrez and Kupinovo is called potkovica. Higher grounds with cut-in depressions and old oak forests are called kopito. A Ramsar Site.</obo:IAO_0000115>
        <oboInOwl:hasOBONamespace>GAZ</oboInOwl:hasOBONamespace>
        <oboInOwl:id>GAZ:00062780</oboInOwl:id>
        <rdfs:label>Obedska bara</rdfs:label>
    </owl:NamedIndividual>
    


    <!-- http://purl.obolibrary.org/obo/GAZ_00062783 -->

    <owl:NamedIndividual rdf:about="http://purl.obolibrary.org/obo/GAZ_00062783">
        <obo:IAO_0000115>The Rzav&apos;s longer headstream. It originates from the Cigota mountain, eastern section of the Zlatibor mountain. The river originally flows northward, next to the villages of Vodice and Jokina Cuprija, reaches the central section of the Zlatibor where it is dammed and creates the artificial Ribnica Lake (surface area of 10 km2), after the nearby village of Ribnica. After the lake, the river sharply turns west and soon gets followed by the parallel stream of the Jablanica river. After crossing the village of Mokra Gora (hamlet Panjak) on the Serbian-Bosnian border Crni Rzav meets the Jablanica river at the village Gornje Vardisse and finally the river Beli Rzav at the village of Donje Vardiste.</obo:IAO_0000115>
        <oboInOwl:hasOBONamespace>GAZ</oboInOwl:hasOBONamespace>
        <oboInOwl:id>GAZ:00062783</oboInOwl:id>
        <rdfs:label>Crni Rzav</rdfs:label>
    </owl:NamedIndividual>
    


    <!-- http://purl.obolibrary.org/obo/GAZ_00062784 -->

    <owl:NamedIndividual rdf:about="http://purl.obolibrary.org/obo/GAZ_00062784">
        <obo:IAO_0000115>The Rzav&apos;s shorter headstream. It originates from the eastern slopes of the Zvijezda mountain, close to the Bosnian border. After it passes the monastery and village of Rastiste, it turns southward to the Tara mountain, receiving many small streams from both Tara and Zvijezda mountains. At the monastery and village of Zaovine, the Beli Rzav is dammed and the artificial Zaovine Lake is created. After crossing the village of Mokra Gora (hamlets Krsanje and Kotroman), the river turns west, enters Bosnia and Herzegovina and right across the border meets the Crni Rzav at the village of Donje Vardiste.</obo:IAO_0000115>
        <oboInOwl:hasOBONamespace>GAZ</oboInOwl:hasOBONamespace>
        <oboInOwl:id>GAZ:00062784</oboInOwl:id>
        <rdfs:label>Beli Rzav</rdfs:label>
    </owl:NamedIndividual>
    


    <!-- http://purl.obolibrary.org/obo/GAZ_00062785 -->

    <owl:NamedIndividual rdf:about="http://purl.obolibrary.org/obo/GAZ_00062785">
        <obo:RO_0001025 rdf:resource="http://purl.obolibrary.org/obo/GAZ_00062783"/>
        <obo:IAO_0000115>A reservoir on the Crni Rzav River.</obo:IAO_0000115>
        <oboInOwl:hasOBONamespace>GAZ</oboInOwl:hasOBONamespace>
        <oboInOwl:id>GAZ:00062785</oboInOwl:id>
        <rdfs:label>Ribnica Lake</rdfs:label>
    </owl:NamedIndividual>
    


    <!-- http://purl.obolibrary.org/obo/GAZ_00062786 -->

    <owl:NamedIndividual rdf:about="http://purl.obolibrary.org/obo/GAZ_00062786">
        <obo:RO_0001025 rdf:resource="http://purl.obolibrary.org/obo/GAZ_00062784"/>
        <obo:IAO_0000115>A reservoir on the Beli Raz River.</obo:IAO_0000115>
        <oboInOwl:hasOBONamespace>GAZ</oboInOwl:hasOBONamespace>
        <oboInOwl:id>GAZ:00062786</oboInOwl:id>
        <rdfs:label>Zaovine Lake</rdfs:label>
    </owl:NamedIndividual>
    


    <!-- http://purl.obolibrary.org/obo/GAZ_00062789 -->

    <owl:NamedIndividual rdf:about="http://purl.obolibrary.org/obo/GAZ_00062789">
        <obo:IAO_0000115>A reservoir on the Drina River in Serbia.</obo:IAO_0000115>
        <oboInOwl:hasOBONamespace>GAZ</oboInOwl:hasOBONamespace>
        <oboInOwl:id>GAZ:00062789</oboInOwl:id>
        <rdfs:label>Lake Perucac</rdfs:label>
    </owl:NamedIndividual>
    


    <!-- http://purl.obolibrary.org/obo/GAZ_00062790 -->

    <owl:NamedIndividual rdf:about="http://purl.obolibrary.org/obo/GAZ_00062790">
        <obo:IAO_0000115>A reservoir on the Drina River in Serbia.</obo:IAO_0000115>
        <oboInOwl:hasOBONamespace>GAZ</oboInOwl:hasOBONamespace>
        <oboInOwl:id>GAZ:00062790</oboInOwl:id>
        <rdfs:label>Lake Zvornik</rdfs:label>
    </owl:NamedIndividual>
    


    <!-- http://purl.obolibrary.org/obo/GAZ_00062791 -->

    <owl:NamedIndividual rdf:about="http://purl.obolibrary.org/obo/GAZ_00062791">
        <obo:IAO_0000115>A river in Serbia, Montenegro and Kosovo, with a total length of 276 km. It starts in eastern Montenegro and flows into the Zapadna Morava, central Serbia, near Kraljevo.</obo:IAO_0000115>
        <oboInOwl:hasOBONamespace>GAZ</oboInOwl:hasOBONamespace>
        <oboInOwl:id>GAZ:00062791</oboInOwl:id>
        <rdfs:label>Ibar</rdfs:label>
    </owl:NamedIndividual>
    


    <!-- http://purl.obolibrary.org/obo/GAZ_00062792 -->

    <owl:NamedIndividual rdf:about="http://purl.obolibrary.org/obo/GAZ_00062792">
        <obo:RO_0001025 rdf:resource="http://purl.obolibrary.org/obo/GAZ_00062791"/>
        <obo:IAO_0000115>A reservoir on the Ibar River in Serbia.</obo:IAO_0000115>
        <oboInOwl:hasOBONamespace>GAZ</oboInOwl:hasOBONamespace>
        <oboInOwl:id>GAZ:00062792</oboInOwl:id>
        <rdfs:label>Lake Gazivode</rdfs:label>
    </owl:NamedIndividual>
    


    <!-- http://purl.obolibrary.org/obo/GAZ_00062793 -->

    <owl:NamedIndividual rdf:about="http://purl.obolibrary.org/obo/GAZ_00062793">
        <obo:RO_0001025 rdf:resource="http://purl.obolibrary.org/obo/GAZ_00062791"/>
        <obo:IAO_0000115>A reservoir on the Ibar River in Serbia.</obo:IAO_0000115>
        <oboInOwl:hasOBONamespace>GAZ</oboInOwl:hasOBONamespace>
        <oboInOwl:id>GAZ:00062793</oboInOwl:id>
        <rdfs:label>Lake Pridvorice</rdfs:label>
    </owl:NamedIndividual>
    


    <!-- http://purl.obolibrary.org/obo/GAZ_00062794 -->

    <owl:NamedIndividual rdf:about="http://purl.obolibrary.org/obo/GAZ_00062794">
        <obo:IAO_0000115>A river in southwestern Serbia and Republika Srpska, Bosnia and Herzegovina, 119 km long right and major tributary of the Lim, loosely making the northern border of the Sandzak/Raska region. Before it empties into the Lim, for a 10 km it forms the border between Serbia and Bosnia and Herzegovina.</obo:IAO_0000115>
        <oboInOwl:hasOBONamespace>GAZ</oboInOwl:hasOBONamespace>
        <oboInOwl:id>GAZ:00062794</oboInOwl:id>
        <rdfs:label>Uvac</rdfs:label>
    </owl:NamedIndividual>
    


    <!-- http://purl.obolibrary.org/obo/GAZ_00062795 -->

    <owl:NamedIndividual rdf:about="http://purl.obolibrary.org/obo/GAZ_00062795">
        <obo:RO_0001025 rdf:resource="http://purl.obolibrary.org/obo/GAZ_00062794"/>
        <obo:IAO_0000115>A reservoir on the Uvac River in Serbia.</obo:IAO_0000115>
        <oboInOwl:hasOBONamespace>GAZ</oboInOwl:hasOBONamespace>
        <oboInOwl:id>GAZ:00062795</oboInOwl:id>
        <rdfs:label>Zlatar Lake</rdfs:label>
    </owl:NamedIndividual>
    


    <!-- http://purl.obolibrary.org/obo/GAZ_00062797 -->

    <owl:NamedIndividual rdf:about="http://purl.obolibrary.org/obo/GAZ_00062797">
        <obo:IAO_0000115>A reservoir on the Lim River in Serbia.</obo:IAO_0000115>
        <oboInOwl:hasOBONamespace>GAZ</oboInOwl:hasOBONamespace>
        <oboInOwl:id>GAZ:00062797</oboInOwl:id>
        <rdfs:label>Potpec Lake</rdfs:label>
    </owl:NamedIndividual>
    


    <!-- http://purl.obolibrary.org/obo/GAZ_00062798 -->

    <owl:NamedIndividual rdf:about="http://purl.obolibrary.org/obo/GAZ_00062798">
        <obo:RO_0001025 rdf:resource="http://purl.obolibrary.org/obo/GAZ_00062794"/>
        <obo:IAO_0000115>A reservoir on the Uvac River in Serbia.</obo:IAO_0000115>
        <oboInOwl:hasOBONamespace>GAZ</oboInOwl:hasOBONamespace>
        <oboInOwl:id>GAZ:00062798</oboInOwl:id>
        <rdfs:label>Sjenica Lake</rdfs:label>
    </owl:NamedIndividual>
    


    <!-- http://purl.obolibrary.org/obo/GAZ_00062802 -->

    <owl:NamedIndividual rdf:about="http://purl.obolibrary.org/obo/GAZ_00062802">
        <obo:IAO_0000115>An artificial lake on the Krivaja River.</obo:IAO_0000115>
        <oboInOwl:hasOBONamespace>GAZ</oboInOwl:hasOBONamespace>
        <oboInOwl:id>GAZ:00062802</oboInOwl:id>
        <rdfs:label>Zobnatica Lake</rdfs:label>
    </owl:NamedIndividual>
    


    <!-- http://purl.obolibrary.org/obo/GAZ_00062805 -->

    <owl:NamedIndividual rdf:about="http://purl.obolibrary.org/obo/GAZ_00062805">
        <obo:IAO_0000115>A river in central Serbia, a 308 km-long headstream of the Great Morava, which it forms with the South Morava.</obo:IAO_0000115>
        <oboInOwl:hasOBONamespace>GAZ</oboInOwl:hasOBONamespace>
        <oboInOwl:id>GAZ:00062805</oboInOwl:id>
        <rdfs:label>Zapadna Morava</rdfs:label>
    </owl:NamedIndividual>
    


    <!-- http://purl.obolibrary.org/obo/GAZ_00062806 -->

    <owl:NamedIndividual rdf:about="http://purl.obolibrary.org/obo/GAZ_00062806">
        <obo:RO_0001025 rdf:resource="http://purl.obolibrary.org/obo/GAZ_00062805"/>
        <obo:IAO_0000115>An artificial lake on the West Morava River.</obo:IAO_0000115>
        <oboInOwl:hasOBONamespace>GAZ</oboInOwl:hasOBONamespace>
        <oboInOwl:id>GAZ:00062806</oboInOwl:id>
        <rdfs:label>Meduvrsje Lake</rdfs:label>
    </owl:NamedIndividual>
    


    <!-- http://purl.obolibrary.org/obo/GAZ_00062807 -->

    <owl:NamedIndividual rdf:about="http://purl.obolibrary.org/obo/GAZ_00062807">
        <obo:RO_0001025 rdf:resource="http://purl.obolibrary.org/obo/GAZ_00062805"/>
        <obo:IAO_0000115>An artificial lake on the West Morava River.</obo:IAO_0000115>
        <oboInOwl:hasOBONamespace>GAZ</oboInOwl:hasOBONamespace>
        <oboInOwl:id>GAZ:00062807</oboInOwl:id>
        <rdfs:label>Ovcar-Kablar Lake</rdfs:label>
    </owl:NamedIndividual>
    


    <!-- http://purl.obolibrary.org/obo/GAZ_00062808 -->

    <owl:NamedIndividual rdf:about="http://purl.obolibrary.org/obo/GAZ_00062808">
        <obo:RO_0001025 rdf:resource="http://purl.obolibrary.org/obo/GAZ_00061994"/>
        <obo:IAO_0000115>A glacial lake situated at 2,034 m of altitude in the Fagaras Mountains, in central Romania, in Sibiu County.</obo:IAO_0000115>
        <oboInOwl:hasOBONamespace>GAZ</oboInOwl:hasOBONamespace>
        <oboInOwl:id>GAZ:00062808</oboInOwl:id>
        <rdfs:label>Lacul Balea</rdfs:label>
    </owl:NamedIndividual>
    


    <!-- http://purl.obolibrary.org/obo/GAZ_00062809 -->

    <owl:NamedIndividual rdf:about="http://purl.obolibrary.org/obo/GAZ_00062809">
        <obo:IAO_0000115>A river in the Romanian region of Moldavia. Near Bacau it flows into the Siret River. It flows through the counties Suceava, Neamt and Bacau. The upper reach of the river is also known as Bistrita Aurie (German: Goldene Bistritz).</obo:IAO_0000115>
        <oboInOwl:hasOBONamespace>GAZ</oboInOwl:hasOBONamespace>
        <oboInOwl:id>GAZ:00062809</oboInOwl:id>
        <rdfs:label>Bistrita</rdfs:label>
    </owl:NamedIndividual>
    


    <!-- http://purl.obolibrary.org/obo/GAZ_00062810 -->

    <owl:NamedIndividual rdf:about="http://purl.obolibrary.org/obo/GAZ_00062810">
        <obo:RO_0001025 rdf:resource="http://purl.obolibrary.org/obo/GAZ_00061962"/>
        <obo:RO_0001025 rdf:resource="http://purl.obolibrary.org/obo/GAZ_00062809"/>
        <obo:IAO_0000115>An artificial lake that was created after the completion of a dam built on the Bistrita River. The dam is located a few km north of the town of Bicaz. The dam was built between 1950 and 1960.</obo:IAO_0000115>
        <oboInOwl:hasOBONamespace>GAZ</oboInOwl:hasOBONamespace>
        <oboInOwl:id>GAZ:00062810</oboInOwl:id>
        <rdfs:label>Lacul Izvorul Muntelui</rdfs:label>
    </owl:NamedIndividual>
    


    <!-- http://purl.obolibrary.org/obo/GAZ_00062814 -->

    <owl:NamedIndividual rdf:about="http://purl.obolibrary.org/obo/GAZ_00062814">
        <obo:RO_0001025 rdf:resource="http://purl.obolibrary.org/obo/GAZ_00042218"/>
        <obo:IAO_0000115>A lake in the Danube Delta.</obo:IAO_0000115>
        <oboInOwl:hasOBONamespace>GAZ</oboInOwl:hasOBONamespace>
        <oboInOwl:id>GAZ:00062814</oboInOwl:id>
        <rdfs:label>Lacul Matita</rdfs:label>
    </owl:NamedIndividual>
    


    <!-- http://purl.obolibrary.org/obo/GAZ_00062815 -->

    <owl:NamedIndividual rdf:about="http://purl.obolibrary.org/obo/GAZ_00062815">
        <obo:RO_0001025 rdf:resource="http://purl.obolibrary.org/obo/GAZ_00042218"/>
        <obo:IAO_0000115>A lake in the Danube Delta.</obo:IAO_0000115>
        <oboInOwl:hasOBONamespace>GAZ</oboInOwl:hasOBONamespace>
        <oboInOwl:id>GAZ:00062815</oboInOwl:id>
        <rdfs:label>Lacul Furtuna</rdfs:label>
    </owl:NamedIndividual>
    


    <!-- http://purl.obolibrary.org/obo/GAZ_00062816 -->

    <owl:NamedIndividual rdf:about="http://purl.obolibrary.org/obo/GAZ_00062816">
        <obo:RO_0001025 rdf:resource="http://purl.obolibrary.org/obo/GAZ_00042218"/>
        <obo:IAO_0000115>A lake in the Danube Delta.</obo:IAO_0000115>
        <oboInOwl:hasOBONamespace>GAZ</oboInOwl:hasOBONamespace>
        <oboInOwl:id>GAZ:00062816</oboInOwl:id>
        <rdfs:label>Lacul Ledeanca</rdfs:label>
    </owl:NamedIndividual>
    


    <!-- http://purl.obolibrary.org/obo/GAZ_00062817 -->

    <owl:NamedIndividual rdf:about="http://purl.obolibrary.org/obo/GAZ_00062817">
        <obo:RO_0001025 rdf:resource="http://purl.obolibrary.org/obo/GAZ_00042218"/>
        <obo:IAO_0000115>A lake in the Danube Delta.</obo:IAO_0000115>
        <oboInOwl:hasOBONamespace>GAZ</oboInOwl:hasOBONamespace>
        <oboInOwl:id>GAZ:00062817</oboInOwl:id>
        <rdfs:label>Lacul Puiu</rdfs:label>
    </owl:NamedIndividual>
    


    <!-- http://purl.obolibrary.org/obo/GAZ_00062818 -->

    <owl:NamedIndividual rdf:about="http://purl.obolibrary.org/obo/GAZ_00062818">
        <obo:RO_0001025 rdf:resource="http://purl.obolibrary.org/obo/GAZ_00042218"/>
        <obo:IAO_0000115>A lake in the Danube Delta.</obo:IAO_0000115>
        <oboInOwl:hasOBONamespace>GAZ</oboInOwl:hasOBONamespace>
        <oboInOwl:id>GAZ:00062818</oboInOwl:id>
        <rdfs:label>Lacul Puiulet</rdfs:label>
    </owl:NamedIndividual>
    


    <!-- http://purl.obolibrary.org/obo/GAZ_00062819 -->

    <owl:NamedIndividual rdf:about="http://purl.obolibrary.org/obo/GAZ_00062819">
        <obo:RO_0001025 rdf:resource="http://purl.obolibrary.org/obo/GAZ_00042218"/>
        <obo:IAO_0000115>A lake in the Danube Delta.</obo:IAO_0000115>
        <oboInOwl:hasOBONamespace>GAZ</oboInOwl:hasOBONamespace>
        <oboInOwl:id>GAZ:00062819</oboInOwl:id>
        <rdfs:label>Lacul Lumina</rdfs:label>
    </owl:NamedIndividual>
    


    <!-- http://purl.obolibrary.org/obo/GAZ_00062820 -->

    <owl:NamedIndividual rdf:about="http://purl.obolibrary.org/obo/GAZ_00062820">
        <obo:RO_0001025 rdf:resource="http://purl.obolibrary.org/obo/GAZ_00042218"/>
        <obo:IAO_0000115>A lake in the Danube Delta.</obo:IAO_0000115>
        <oboInOwl:hasOBONamespace>GAZ</oboInOwl:hasOBONamespace>
        <oboInOwl:id>GAZ:00062820</oboInOwl:id>
        <rdfs:label>Lacul Uzlina</rdfs:label>
    </owl:NamedIndividual>
    


    <!-- http://purl.obolibrary.org/obo/GAZ_00062821 -->

    <owl:NamedIndividual rdf:about="http://purl.obolibrary.org/obo/GAZ_00062821">
        <obo:RO_0001025 rdf:resource="http://purl.obolibrary.org/obo/GAZ_00042218"/>
        <obo:IAO_0000115>A lake in the Danube Delta.</obo:IAO_0000115>
        <oboInOwl:hasOBONamespace>GAZ</oboInOwl:hasOBONamespace>
        <oboInOwl:id>GAZ:00062821</oboInOwl:id>
        <rdfs:label>Lacul Dranov</rdfs:label>
    </owl:NamedIndividual>
    


    <!-- http://purl.obolibrary.org/obo/GAZ_00062822 -->

    <owl:NamedIndividual rdf:about="http://purl.obolibrary.org/obo/GAZ_00062822">
        <obo:RO_0001025 rdf:resource="http://purl.obolibrary.org/obo/GAZ_00042218"/>
        <obo:IAO_0000115>A lake in the Danube Delta.</obo:IAO_0000115>
        <oboInOwl:hasOBONamespace>GAZ</oboInOwl:hasOBONamespace>
        <oboInOwl:id>GAZ:00062822</oboInOwl:id>
        <rdfs:label>Lacul Tatanir</rdfs:label>
    </owl:NamedIndividual>
    


    <!-- http://purl.obolibrary.org/obo/GAZ_00062823 -->

    <owl:NamedIndividual rdf:about="http://purl.obolibrary.org/obo/GAZ_00062823">
        <obo:RO_0001025 rdf:resource="http://purl.obolibrary.org/obo/GAZ_00042218"/>
        <obo:IAO_0000115>A lake in the Danube Delta.</obo:IAO_0000115>
        <oboInOwl:hasOBONamespace>GAZ</oboInOwl:hasOBONamespace>
        <oboInOwl:id>GAZ:00062823</oboInOwl:id>
        <rdfs:label>Lacul Gorgova</rdfs:label>
    </owl:NamedIndividual>
    


    <!-- http://purl.obolibrary.org/obo/GAZ_00062824 -->

    <owl:NamedIndividual rdf:about="http://purl.obolibrary.org/obo/GAZ_00062824">
        <obo:RO_0001025 rdf:resource="http://purl.obolibrary.org/obo/GAZ_00042218"/>
        <obo:IAO_0000115>A lake in the Danube Delta.</obo:IAO_0000115>
        <oboInOwl:hasOBONamespace>GAZ</oboInOwl:hasOBONamespace>
        <oboInOwl:id>GAZ:00062824</oboInOwl:id>
        <rdfs:label>Lacul Merhel</rdfs:label>
    </owl:NamedIndividual>
    


    <!-- http://purl.obolibrary.org/obo/GAZ_00062825 -->

    <owl:NamedIndividual rdf:about="http://purl.obolibrary.org/obo/GAZ_00062825">
        <obo:RO_0001025 rdf:resource="http://purl.obolibrary.org/obo/GAZ_00042218"/>
        <obo:IAO_0000115>A lake in the Danube Delta.</obo:IAO_0000115>
        <oboInOwl:hasOBONamespace>GAZ</oboInOwl:hasOBONamespace>
        <oboInOwl:id>GAZ:00062825</oboInOwl:id>
        <rdfs:label>Lacul Isac</rdfs:label>
    </owl:NamedIndividual>
    


    <!-- http://purl.obolibrary.org/obo/GAZ_00062826 -->

    <owl:NamedIndividual rdf:about="http://purl.obolibrary.org/obo/GAZ_00062826">
        <obo:RO_0001025 rdf:resource="http://purl.obolibrary.org/obo/GAZ_00042218"/>
        <obo:IAO_0000115>A lake in the Danube Delta.</obo:IAO_0000115>
        <oboInOwl:hasOBONamespace>GAZ</oboInOwl:hasOBONamespace>
        <oboInOwl:id>GAZ:00062826</oboInOwl:id>
        <rdfs:label>Lacul Rosu</rdfs:label>
    </owl:NamedIndividual>
    


    <!-- http://purl.obolibrary.org/obo/GAZ_00062827 -->

    <owl:NamedIndividual rdf:about="http://purl.obolibrary.org/obo/GAZ_00062827">
        <obo:RO_0001025 rdf:resource="http://purl.obolibrary.org/obo/GAZ_00042218"/>
        <oboInOwl:hasOBONamespace>GAZ</oboInOwl:hasOBONamespace>
        <oboInOwl:id>GAZ:00062827</oboInOwl:id>
        <rdfs:label>Tulcea Arm</rdfs:label>
    </owl:NamedIndividual>
    


    <!-- http://purl.obolibrary.org/obo/GAZ_00062829 -->

    <owl:NamedIndividual rdf:about="http://purl.obolibrary.org/obo/GAZ_00062829">
        <obo:RO_0001025 rdf:resource="http://purl.obolibrary.org/obo/GAZ_00061963"/>
        <obo:IAO_0000115>A lake in the Eastern Carpathians chain in Harghita County, Romania.</obo:IAO_0000115>
        <oboInOwl:hasOBONamespace>GAZ</oboInOwl:hasOBONamespace>
        <oboInOwl:id>GAZ:00062829</oboInOwl:id>
        <rdfs:label>Lacul Rosu</rdfs:label>
    </owl:NamedIndividual>
    


    <!-- http://purl.obolibrary.org/obo/GAZ_00062830 -->

    <owl:NamedIndividual rdf:about="http://purl.obolibrary.org/obo/GAZ_00062830">
        <obo:RO_0001025 rdf:resource="http://purl.obolibrary.org/obo/GAZ_00061908"/>
        <obo:IAO_0000115>A crater lake located in the volcanic crater named &quot;Puciosul&quot; of the Eastern Carpathians, near Tusnad in the Natural Reserve of Mohos, Harghita County, Romania.</obo:IAO_0000115>
        <oboInOwl:hasOBONamespace>GAZ</oboInOwl:hasOBONamespace>
        <oboInOwl:id>GAZ:00062830</oboInOwl:id>
        <rdfs:label>Lacul Sfanta Ana</rdfs:label>
    </owl:NamedIndividual>
    


    <!-- http://purl.obolibrary.org/obo/GAZ_00062839 -->

    <owl:NamedIndividual rdf:about="http://purl.obolibrary.org/obo/GAZ_00062839">
        <obo:IAO_0000115>An artificial lake in Romania. It was created in 1965 by the construction of the Vidraru Dam on the Arges River.</obo:IAO_0000115>
        <oboInOwl:hasOBONamespace>GAZ</oboInOwl:hasOBONamespace>
        <oboInOwl:id>GAZ:00062839</oboInOwl:id>
        <rdfs:label>Lacul Vidraru</rdfs:label>
    </owl:NamedIndividual>
    


    <!-- http://purl.obolibrary.org/obo/GAZ_00062841 -->

    <owl:NamedIndividual rdf:about="http://purl.obolibrary.org/obo/GAZ_00062841">
        <obo:RO_0001025 rdf:resource="http://purl.obolibrary.org/obo/GAZ_00061915"/>
        <obo:IAO_0000115>A periglacial lake located in the Buzau Mountains, at the Carpathian Mountains south-eastern curvature, at an altitude of 1420 m. The nearest town is Siriu.</obo:IAO_0000115>
        <oboInOwl:hasOBONamespace>GAZ</oboInOwl:hasOBONamespace>
        <oboInOwl:id>GAZ:00062841</oboInOwl:id>
        <rdfs:label>Lacul Vulturilor</rdfs:label>
    </owl:NamedIndividual>
    


    <!-- http://purl.obolibrary.org/obo/GAZ_00062842 -->

    <owl:NamedIndividual rdf:about="http://purl.obolibrary.org/obo/GAZ_00062842">
        <obo:RO_0001025 rdf:resource="http://purl.obolibrary.org/obo/GAZ_00061993"/>
        <obo:RO_0001025 rdf:resource="http://purl.obolibrary.org/obo/GAZ_00062006"/>
        <obo:IAO_0000115>A glacial lake in the Lotru River basin, Romania.</obo:IAO_0000115>
        <oboInOwl:hasOBONamespace>GAZ</oboInOwl:hasOBONamespace>
        <oboInOwl:id>GAZ:00062842</oboInOwl:id>
        <rdfs:label>Lacul Zanoaga Mare</rdfs:label>
    </owl:NamedIndividual>
    


    <!-- http://purl.obolibrary.org/obo/GAZ_00062864 -->

    <owl:NamedIndividual rdf:about="http://purl.obolibrary.org/obo/GAZ_00062864">
        <obo:IAO_0000115>An island.</obo:IAO_0000115>
        <oboInOwl:hasOBONamespace>GAZ</oboInOwl:hasOBONamespace>
        <oboInOwl:id>GAZ:00062864</oboInOwl:id>
        <rdfs:label>Ostrovu Mare</rdfs:label>
    </owl:NamedIndividual>
    


    <!-- http://purl.obolibrary.org/obo/GAZ_00062872 -->

    <owl:NamedIndividual rdf:about="http://purl.obolibrary.org/obo/GAZ_00062872">
        <obo:RO_0001025 rdf:resource="http://purl.obolibrary.org/obo/GAZ_00062022"/>
        <obo:IAO_0000115>An artificial lake.</obo:IAO_0000115>
        <oboInOwl:hasOBONamespace>GAZ</oboInOwl:hasOBONamespace>
        <oboInOwl:id>GAZ:00062872</oboInOwl:id>
        <rdfs:label>Lacul Fantanele</rdfs:label>
    </owl:NamedIndividual>
    


    <!-- http://purl.obolibrary.org/obo/GAZ_00062873 -->

    <owl:NamedIndividual rdf:about="http://purl.obolibrary.org/obo/GAZ_00062873">
        <obo:RO_0001025 rdf:resource="http://purl.obolibrary.org/obo/GAZ_00061709"/>
        <obo:IAO_0000115>A reservoir.</obo:IAO_0000115>
        <oboInOwl:hasOBONamespace>GAZ</oboInOwl:hasOBONamespace>
        <oboInOwl:id>GAZ:00062873</oboInOwl:id>
        <rdfs:label>Lacul de acumulare Vidra</rdfs:label>
    </owl:NamedIndividual>
    


    <!-- http://purl.obolibrary.org/obo/GAZ_00062875 -->

    <owl:NamedIndividual rdf:about="http://purl.obolibrary.org/obo/GAZ_00062875">
        <obo:RO_0001025 rdf:resource="http://purl.obolibrary.org/obo/GAZ_00062022"/>
        <obo:IAO_0000115>A storage reservoir in the Somesul Cald River basin, Romania.</obo:IAO_0000115>
        <oboInOwl:hasOBONamespace>GAZ</oboInOwl:hasOBONamespace>
        <oboInOwl:id>GAZ:00062875</oboInOwl:id>
        <rdfs:label>Fantanele</rdfs:label>
    </owl:NamedIndividual>
    


    <!-- http://purl.obolibrary.org/obo/GAZ_00062876 -->

    <owl:NamedIndividual rdf:about="http://purl.obolibrary.org/obo/GAZ_00062876">
        <obo:RO_0001025 rdf:resource="http://purl.obolibrary.org/obo/GAZ_00061994"/>
        <obo:IAO_0000115>A lake in Romania.</obo:IAO_0000115>
        <oboInOwl:hasOBONamespace>GAZ</oboInOwl:hasOBONamespace>
        <oboInOwl:id>GAZ:00062876</oboInOwl:id>
        <rdfs:label>Vidraru</rdfs:label>
    </owl:NamedIndividual>
    


    <!-- http://purl.obolibrary.org/obo/GAZ_00062879 -->

    <owl:NamedIndividual rdf:about="http://purl.obolibrary.org/obo/GAZ_00062879">
        <rdf:type rdf:resource="http://purl.obolibrary.org/obo/ENVO_00000104"/>
        <obo:IAO_0000115>A large basin in Central Europe. The basin forms a topographically discrete unit set in the European landscape, surrounded by imposing geographic boundaries that have created a fairly unified cultural area that looks more towards the south and east than to the north and west. The river Danube divides the basin roughly in half. The Pannonian Plain is a large plain in Central Europe that remained when the Pliocene Pannonian Sea dried out. It is a geomorphological subsystem of the Alps-Himalaya system. The plain is roughly bounded by the Carpathian mountains, the Alps, the Dinaric Alps and the Balkan mountains.</obo:IAO_0000115>
        <oboInOwl:hasOBONamespace>GAZ</oboInOwl:hasOBONamespace>
        <oboInOwl:id>GAZ:00062879</oboInOwl:id>
        <rdfs:label>Pannonian Plain</rdfs:label>
    </owl:NamedIndividual>
    


    <!-- http://purl.obolibrary.org/obo/GAZ_00062880 -->

    <owl:NamedIndividual rdf:about="http://purl.obolibrary.org/obo/GAZ_00062880">
        <obo:RO_0001025 rdf:resource="http://purl.obolibrary.org/obo/GAZ_00062879"/>
        <obo:IAO_0000115>A plain (tectonic basin) of about 8,000 km2 in northwestern Hungary, south-western Slovakia, and eastern Austria. It is a part of the Pannonian plain which covers most parts of Hungary. Its borders are the Carpathians on the north, the Bakony-Vertes Hills (at the Balaton) in the south, and the Vienna Basin and the Alps in the west. In Hungary, it includes most of Gyor-Moson-Sopron and Vas counties, and the western part of Komarom-Esztergom and Veszprem. The plain is roughly cut in half by the Danube which is split up into many arms between Bratislava and Komarno, forming large islands.</obo:IAO_0000115>
        <oboInOwl:hasOBONamespace>GAZ</oboInOwl:hasOBONamespace>
        <oboInOwl:id>GAZ:00062880</oboInOwl:id>
        <rdfs:label>Little Hungarian Plain</rdfs:label>
    </owl:NamedIndividual>
    


    <!-- http://purl.obolibrary.org/obo/GAZ_00062881 -->

    <owl:NamedIndividual rdf:about="http://purl.obolibrary.org/obo/GAZ_00062881">
        <obo:RO_0001025 rdf:resource="http://purl.obolibrary.org/obo/GAZ_00062879"/>
        <obo:IAO_0000115>A plain occupying the southern and eastern part of Hungary, some parts of eastern Slovakia, southwestern Ukraine, western Romania, northern Serbia and eastern Croatia. It is the largest part of the Pannonian Plain. Its boundaries are the Carpathians in the north and east, the Transdanubian Medium Mountains and Croatian mountains in the southwest, and approximately the Sava river in the south.</obo:IAO_0000115>
        <oboInOwl:hasOBONamespace>GAZ</oboInOwl:hasOBONamespace>
        <oboInOwl:id>GAZ:00062881</oboInOwl:id>
        <rdfs:label>Great Hungarian Plain</rdfs:label>
    </owl:NamedIndividual>
    


    <!-- http://purl.obolibrary.org/obo/GAZ_00062882 -->

    <owl:NamedIndividual rdf:about="http://purl.obolibrary.org/obo/GAZ_00062882">
        <obo:RO_0001025 rdf:resource="http://purl.obolibrary.org/obo/GAZ_00061961"/>
        <obo:IAO_0000115>A storage reservoir in the Sasar River basin (Romania).</obo:IAO_0000115>
        <oboInOwl:hasOBONamespace>GAZ</oboInOwl:hasOBONamespace>
        <oboInOwl:id>GAZ:00062882</oboInOwl:id>
        <rdfs:label>Bodi II</rdfs:label>
    </owl:NamedIndividual>
    


    <!-- http://purl.obolibrary.org/obo/GAZ_00062883 -->

    <owl:NamedIndividual rdf:about="http://purl.obolibrary.org/obo/GAZ_00062883">
        <obo:RO_0001025 rdf:resource="http://purl.obolibrary.org/obo/GAZ_00061961"/>
        <obo:IAO_0000115>A storage reservoir in the Sasar River basin (Romania).</obo:IAO_0000115>
        <oboInOwl:hasOBONamespace>GAZ</oboInOwl:hasOBONamespace>
        <oboInOwl:id>GAZ:00062883</oboInOwl:id>
        <rdfs:label>Bodi-Ferneziu</rdfs:label>
    </owl:NamedIndividual>
    


    <!-- http://purl.obolibrary.org/obo/GAZ_00062884 -->

    <owl:NamedIndividual rdf:about="http://purl.obolibrary.org/obo/GAZ_00062884">
        <obo:RO_0001025 rdf:resource="http://purl.obolibrary.org/obo/GAZ_00061961"/>
        <obo:IAO_0000115>A storage reservoir in the Sasar River basin (Romania).</obo:IAO_0000115>
        <oboInOwl:hasOBONamespace>GAZ</oboInOwl:hasOBONamespace>
        <oboInOwl:id>GAZ:00062884</oboInOwl:id>
        <rdfs:label>Firiza</rdfs:label>
    </owl:NamedIndividual>
    


    <!-- http://purl.obolibrary.org/obo/GAZ_00062885 -->

    <owl:NamedIndividual rdf:about="http://purl.obolibrary.org/obo/GAZ_00062885">
        <obo:RO_0001025 rdf:resource="http://purl.obolibrary.org/obo/GAZ_00061961"/>
        <obo:IAO_0000115>A storage reservoir in the Lapus River basin (Romania).</obo:IAO_0000115>
        <oboInOwl:hasOBONamespace>GAZ</oboInOwl:hasOBONamespace>
        <oboInOwl:id>GAZ:00062885</oboInOwl:id>
        <rdfs:label>Lighet</rdfs:label>
    </owl:NamedIndividual>
    


    <!-- http://purl.obolibrary.org/obo/GAZ_00062886 -->

    <owl:NamedIndividual rdf:about="http://purl.obolibrary.org/obo/GAZ_00062886">
        <obo:RO_0001025 rdf:resource="http://purl.obolibrary.org/obo/GAZ_00061961"/>
        <obo:IAO_0000115>A storage reservoir in the Sasar River basin (Romania).</obo:IAO_0000115>
        <oboInOwl:hasOBONamespace>GAZ</oboInOwl:hasOBONamespace>
        <oboInOwl:id>GAZ:00062886</oboInOwl:id>
        <rdfs:label>Nistru</rdfs:label>
    </owl:NamedIndividual>
    


    <!-- http://purl.obolibrary.org/obo/GAZ_00062887 -->

    <owl:NamedIndividual rdf:about="http://purl.obolibrary.org/obo/GAZ_00062887">
        <obo:RO_0001025 rdf:resource="http://purl.obolibrary.org/obo/GAZ_00061961"/>
        <obo:IAO_0000115>A storage reservoir in the Sasar River basin (Romania).</obo:IAO_0000115>
        <oboInOwl:hasOBONamespace>GAZ</oboInOwl:hasOBONamespace>
        <oboInOwl:id>GAZ:00062887</oboInOwl:id>
        <rdfs:label>Bodi I</rdfs:label>
    </owl:NamedIndividual>
    


    <!-- http://purl.obolibrary.org/obo/GAZ_00062888 -->

    <owl:NamedIndividual rdf:about="http://purl.obolibrary.org/obo/GAZ_00062888">
        <obo:RO_0001025 rdf:resource="http://purl.obolibrary.org/obo/GAZ_00061956"/>
        <obo:IAO_0000115>A storage reservoir in theTurulung River basin (Romania).</obo:IAO_0000115>
        <oboInOwl:hasOBONamespace>GAZ</oboInOwl:hasOBONamespace>
        <oboInOwl:id>GAZ:00062888</oboInOwl:id>
        <rdfs:label>Calinesti</rdfs:label>
    </owl:NamedIndividual>
    


    <!-- http://purl.obolibrary.org/obo/GAZ_00062889 -->

    <owl:NamedIndividual rdf:about="http://purl.obolibrary.org/obo/GAZ_00062889">
        <obo:RO_0001025 rdf:resource="http://purl.obolibrary.org/obo/GAZ_00061979"/>
        <obo:IAO_0000115>A lake in the Ruscova-Viseu River basin (Romania).</obo:IAO_0000115>
        <oboInOwl:hasOBONamespace>GAZ</oboInOwl:hasOBONamespace>
        <oboInOwl:id>GAZ:00062889</oboInOwl:id>
        <rdfs:label>Vinderel</rdfs:label>
    </owl:NamedIndividual>
    


    <!-- http://purl.obolibrary.org/obo/GAZ_00062890 -->

    <owl:NamedIndividual rdf:about="http://purl.obolibrary.org/obo/GAZ_00062890">
        <obo:RO_0001025 rdf:resource="http://purl.obolibrary.org/obo/GAZ_00387021"/>
        <obo:IAO_0000115>A glacial lake in the Viseu River basin, Romania.</obo:IAO_0000115>
        <oboInOwl:hasOBONamespace>GAZ</oboInOwl:hasOBONamespace>
        <oboInOwl:id>GAZ:00062890</oboInOwl:id>
        <rdfs:label>Buhaiescu II</rdfs:label>
    </owl:NamedIndividual>
    


    <!-- http://purl.obolibrary.org/obo/GAZ_00062892 -->

    <owl:NamedIndividual rdf:about="http://purl.obolibrary.org/obo/GAZ_00062892">
        <obo:RO_0001025 rdf:resource="http://purl.obolibrary.org/obo/GAZ_00387026"/>
        <obo:IAO_0000115>A glacial lake in the Bistrita River basin, Romania.</obo:IAO_0000115>
        <oboInOwl:hasOBONamespace>GAZ</oboInOwl:hasOBONamespace>
        <oboInOwl:id>GAZ:00062892</oboInOwl:id>
        <rdfs:label>Lacul Lala Mare</rdfs:label>
    </owl:NamedIndividual>
    


    <!-- http://purl.obolibrary.org/obo/GAZ_00062893 -->

    <owl:NamedIndividual rdf:about="http://purl.obolibrary.org/obo/GAZ_00062893">
        <obo:RO_0001025 rdf:resource="http://purl.obolibrary.org/obo/GAZ_00387021"/>
        <obo:IAO_0000115>A glacial lake in the Viseu River basin, Romania.</obo:IAO_0000115>
        <oboInOwl:hasOBONamespace>GAZ</oboInOwl:hasOBONamespace>
        <oboInOwl:id>GAZ:00062893</oboInOwl:id>
        <rdfs:label>Buhaiescu I</rdfs:label>
    </owl:NamedIndividual>
    


    <!-- http://purl.obolibrary.org/obo/GAZ_00062894 -->

    <owl:NamedIndividual rdf:about="http://purl.obolibrary.org/obo/GAZ_00062894">
        <obo:RO_0001025 rdf:resource="http://purl.obolibrary.org/obo/GAZ_00387021"/>
        <obo:IAO_0000115>A glacial lake in the Viseu River basin, Romania.</obo:IAO_0000115>
        <oboInOwl:hasOBONamespace>GAZ</oboInOwl:hasOBONamespace>
        <oboInOwl:id>GAZ:00062894</oboInOwl:id>
        <rdfs:label>Buhaiescu III</rdfs:label>
    </owl:NamedIndividual>
    


    <!-- http://purl.obolibrary.org/obo/GAZ_00062895 -->

    <owl:NamedIndividual rdf:about="http://purl.obolibrary.org/obo/GAZ_00062895">
        <obo:RO_0001025 rdf:resource="http://purl.obolibrary.org/obo/GAZ_00061909"/>
        <obo:IAO_0000115>A lake in the Moldiva River basin, Romania.</obo:IAO_0000115>
        <oboInOwl:hasOBONamespace>GAZ</oboInOwl:hasOBONamespace>
        <oboInOwl:id>GAZ:00062895</oboInOwl:id>
        <rdfs:label>Sadova</rdfs:label>
    </owl:NamedIndividual>
    


    <!-- http://purl.obolibrary.org/obo/GAZ_00062896 -->

    <owl:NamedIndividual rdf:about="http://purl.obolibrary.org/obo/GAZ_00062896">
        <obo:RO_0001025 rdf:resource="http://purl.obolibrary.org/obo/GAZ_00061971"/>
        <obo:IAO_0000115>A lake in the Ilva-Somes River basin, Romania.</obo:IAO_0000115>
        <oboInOwl:hasOBONamespace>GAZ</oboInOwl:hasOBONamespace>
        <oboInOwl:id>GAZ:00062896</oboInOwl:id>
        <rdfs:label>Izvorul Magurii</rdfs:label>
    </owl:NamedIndividual>
    


    <!-- http://purl.obolibrary.org/obo/GAZ_00062897 -->

    <owl:NamedIndividual rdf:about="http://purl.obolibrary.org/obo/GAZ_00062897">
        <obo:RO_0001025 rdf:resource="http://purl.obolibrary.org/obo/GAZ_00061971"/>
        <obo:IAO_0000115>A lake in the Colibita River basin, Romania.</obo:IAO_0000115>
        <oboInOwl:hasOBONamespace>GAZ</oboInOwl:hasOBONamespace>
        <oboInOwl:id>GAZ:00062897</oboInOwl:id>
        <rdfs:label>Zanelor</rdfs:label>
    </owl:NamedIndividual>
    


    <!-- http://purl.obolibrary.org/obo/GAZ_00062898 -->

    <owl:NamedIndividual rdf:about="http://purl.obolibrary.org/obo/GAZ_00062898">
        <obo:RO_0001025 rdf:resource="http://purl.obolibrary.org/obo/GAZ_00061970"/>
        <obo:IAO_0000115>A lake in the Topita-Mures River basin, Romania.</obo:IAO_0000115>
        <oboInOwl:hasOBONamespace>GAZ</oboInOwl:hasOBONamespace>
        <oboInOwl:id>GAZ:00062898</oboInOwl:id>
        <rdfs:label>Racicis</rdfs:label>
    </owl:NamedIndividual>
    


    <!-- http://purl.obolibrary.org/obo/GAZ_00062899 -->

    <owl:NamedIndividual rdf:about="http://purl.obolibrary.org/obo/GAZ_00062899">
        <obo:RO_0001025 rdf:resource="http://purl.obolibrary.org/obo/GAZ_00061914"/>
        <obo:IAO_0000115>A lake in the Bistrita River basin, Romania.</obo:IAO_0000115>
        <oboInOwl:hasOBONamespace>GAZ</oboInOwl:hasOBONamespace>
        <oboInOwl:id>GAZ:00062899</oboInOwl:id>
        <rdfs:label>Batca Doamnei</rdfs:label>
    </owl:NamedIndividual>
    


    <!-- http://purl.obolibrary.org/obo/GAZ_00062900 -->

    <owl:NamedIndividual rdf:about="http://purl.obolibrary.org/obo/GAZ_00062900">
        <obo:RO_0001025 rdf:resource="http://purl.obolibrary.org/obo/GAZ_00061914"/>
        <obo:IAO_0000115>A lake in the Bistrita River basin, Romania.</obo:IAO_0000115>
        <oboInOwl:hasOBONamespace>GAZ</oboInOwl:hasOBONamespace>
        <oboInOwl:id>GAZ:00062900</oboInOwl:id>
        <rdfs:label>Piatra Neamt</rdfs:label>
    </owl:NamedIndividual>
    


    <!-- http://purl.obolibrary.org/obo/GAZ_00062901 -->

    <owl:NamedIndividual rdf:about="http://purl.obolibrary.org/obo/GAZ_00062901">
        <obo:RO_0001025 rdf:resource="http://purl.obolibrary.org/obo/GAZ_00061914"/>
        <obo:IAO_0000115>A lake in the Bistrita River basin, Romania.</obo:IAO_0000115>
        <oboInOwl:hasOBONamespace>GAZ</oboInOwl:hasOBONamespace>
        <oboInOwl:id>GAZ:00062901</oboInOwl:id>
        <rdfs:label>Pangarati</rdfs:label>
    </owl:NamedIndividual>
    


    <!-- http://purl.obolibrary.org/obo/GAZ_00062902 -->

    <owl:NamedIndividual rdf:about="http://purl.obolibrary.org/obo/GAZ_00062902">
        <obo:RO_0001025 rdf:resource="http://purl.obolibrary.org/obo/GAZ_00061914"/>
        <obo:IAO_0000115>A lake in the Bistrita River basin, Romania.</obo:IAO_0000115>
        <oboInOwl:hasOBONamespace>GAZ</oboInOwl:hasOBONamespace>
        <oboInOwl:id>GAZ:00062902</oboInOwl:id>
        <rdfs:label>Vaduri</rdfs:label>
    </owl:NamedIndividual>
    


    <!-- http://purl.obolibrary.org/obo/GAZ_00062903 -->

    <owl:NamedIndividual rdf:about="http://purl.obolibrary.org/obo/GAZ_00062903">
        <obo:RO_0001025 rdf:resource="http://purl.obolibrary.org/obo/GAZ_00061963"/>
        <obo:IAO_0000115>A lake in the Bicaz River basin, Romania.</obo:IAO_0000115>
        <oboInOwl:hasOBONamespace>GAZ</oboInOwl:hasOBONamespace>
        <oboInOwl:id>GAZ:00062903</oboInOwl:id>
        <rdfs:label>Paraul Rosu</rdfs:label>
    </owl:NamedIndividual>
    


    <!-- http://purl.obolibrary.org/obo/GAZ_00062904 -->

    <owl:NamedIndividual rdf:about="http://purl.obolibrary.org/obo/GAZ_00062904">
        <obo:RO_0001025 rdf:resource="http://purl.obolibrary.org/obo/GAZ_00061963"/>
        <obo:IAO_0000115>A lake in the Olt River basin, Romania.</obo:IAO_0000115>
        <oboInOwl:hasOBONamespace>GAZ</oboInOwl:hasOBONamespace>
        <oboInOwl:id>GAZ:00062904</oboInOwl:id>
        <rdfs:label>Mesteacan</rdfs:label>
    </owl:NamedIndividual>
    


    <!-- http://purl.obolibrary.org/obo/GAZ_00062905 -->

    <owl:NamedIndividual rdf:about="http://purl.obolibrary.org/obo/GAZ_00062905">
        <obo:RO_0001025 rdf:resource="http://purl.obolibrary.org/obo/GAZ_00061963"/>
        <obo:IAO_0000115>A lake in the Bicaz River basin, Romania.</obo:IAO_0000115>
        <oboInOwl:hasOBONamespace>GAZ</oboInOwl:hasOBONamespace>
        <oboInOwl:id>GAZ:00062905</oboInOwl:id>
        <rdfs:label>Lacu Oii</rdfs:label>
    </owl:NamedIndividual>
    


    <!-- http://purl.obolibrary.org/obo/GAZ_00062906 -->

    <owl:NamedIndividual rdf:about="http://purl.obolibrary.org/obo/GAZ_00062906">
        <obo:RO_0001025 rdf:resource="http://purl.obolibrary.org/obo/GAZ_00061908"/>
        <obo:IAO_0000115>A lake in the Uz-Trotus River basin, Romania.</obo:IAO_0000115>
        <oboInOwl:hasOBONamespace>GAZ</oboInOwl:hasOBONamespace>
        <oboInOwl:id>GAZ:00062906</oboInOwl:id>
        <rdfs:label>Poiana Uzului</rdfs:label>
    </owl:NamedIndividual>
    


    <!-- http://purl.obolibrary.org/obo/GAZ_00062907 -->

    <owl:NamedIndividual rdf:about="http://purl.obolibrary.org/obo/GAZ_00062907">
        <obo:RO_0001025 rdf:resource="http://purl.obolibrary.org/obo/GAZ_00061908"/>
        <obo:IAO_0000115>A lake in the Uz-Trotus River basin, Romania.</obo:IAO_0000115>
        <oboInOwl:hasOBONamespace>GAZ</oboInOwl:hasOBONamespace>
        <oboInOwl:id>GAZ:00062907</oboInOwl:id>
        <rdfs:label>Lacul Balatau</rdfs:label>
    </owl:NamedIndividual>
    


    <!-- http://purl.obolibrary.org/obo/GAZ_00062908 -->

    <owl:NamedIndividual rdf:about="http://purl.obolibrary.org/obo/GAZ_00062908">
        <obo:RO_0001025 rdf:resource="http://purl.obolibrary.org/obo/GAZ_00061911"/>
        <obo:IAO_0000115>A lake in the Susita River basin, Romania.</obo:IAO_0000115>
        <oboInOwl:hasOBONamespace>GAZ</oboInOwl:hasOBONamespace>
        <oboInOwl:id>GAZ:00062908</oboInOwl:id>
        <rdfs:label>Lacu Verde</rdfs:label>
    </owl:NamedIndividual>
    


    <!-- http://purl.obolibrary.org/obo/GAZ_00062909 -->

    <owl:NamedIndividual rdf:about="http://purl.obolibrary.org/obo/GAZ_00062909">
        <obo:RO_0001025 rdf:resource="http://purl.obolibrary.org/obo/GAZ_00061915"/>
        <obo:IAO_0000115>A lake in the Basca Rosilei River basin, Romania.</obo:IAO_0000115>
        <oboInOwl:hasOBONamespace>GAZ</oboInOwl:hasOBONamespace>
        <oboInOwl:id>GAZ:00062909</oboInOwl:id>
        <rdfs:label>Hansaru</rdfs:label>
    </owl:NamedIndividual>
    


    <!-- http://purl.obolibrary.org/obo/GAZ_00062910 -->

    <owl:NamedIndividual rdf:about="http://purl.obolibrary.org/obo/GAZ_00062910">
        <obo:RO_0001025 rdf:resource="http://purl.obolibrary.org/obo/GAZ_00061915"/>
        <obo:IAO_0000115>A lake in the Slanic River basin, Romania.</obo:IAO_0000115>
        <oboInOwl:hasOBONamespace>GAZ</oboInOwl:hasOBONamespace>
        <oboInOwl:id>GAZ:00062910</oboInOwl:id>
        <rdfs:label>Mocearu</rdfs:label>
    </owl:NamedIndividual>
    


    <!-- http://purl.obolibrary.org/obo/GAZ_00062912 -->

    <owl:NamedIndividual rdf:about="http://purl.obolibrary.org/obo/GAZ_00062912">
        <obo:RO_0001025 rdf:resource="http://purl.obolibrary.org/obo/GAZ_00061915"/>
        <obo:IAO_0000115>A lake in the Basca Mica River basin, Romania.</obo:IAO_0000115>
        <oboInOwl:hasOBONamespace>GAZ</oboInOwl:hasOBONamespace>
        <oboInOwl:id>GAZ:00062912</oboInOwl:id>
        <rdfs:label>Lacul Negru</rdfs:label>
    </owl:NamedIndividual>
    


    <!-- http://purl.obolibrary.org/obo/GAZ_00062913 -->

    <owl:NamedIndividual rdf:about="http://purl.obolibrary.org/obo/GAZ_00062913">
        <obo:RO_0001025 rdf:resource="http://purl.obolibrary.org/obo/GAZ_00061950"/>
        <obo:IAO_0000115>A lake in the Olt River basin, Romania.</obo:IAO_0000115>
        <oboInOwl:hasOBONamespace>GAZ</oboInOwl:hasOBONamespace>
        <oboInOwl:id>GAZ:00062913</oboInOwl:id>
        <rdfs:label>Tarlung</rdfs:label>
    </owl:NamedIndividual>
    


    <!-- http://purl.obolibrary.org/obo/GAZ_00062914 -->

    <owl:NamedIndividual rdf:about="http://purl.obolibrary.org/obo/GAZ_00062914">
        <obo:RO_0001025 rdf:resource="http://purl.obolibrary.org/obo/GAZ_00061950"/>
        <obo:IAO_0000115>A lake in the Doftana River basin, Romania.</obo:IAO_0000115>
        <oboInOwl:hasOBONamespace>GAZ</oboInOwl:hasOBONamespace>
        <oboInOwl:id>GAZ:00062914</oboInOwl:id>
        <rdfs:label>Paltinu</rdfs:label>
    </owl:NamedIndividual>
    


    <!-- http://purl.obolibrary.org/obo/GAZ_00062915 -->

    <owl:NamedIndividual rdf:about="http://purl.obolibrary.org/obo/GAZ_00062915">
        <obo:RO_0001025 rdf:resource="http://purl.obolibrary.org/obo/GAZ_00061983"/>
        <obo:IAO_0000115>A lake in the Ialomita River basin, Romania.</obo:IAO_0000115>
        <oboInOwl:hasOBONamespace>GAZ</oboInOwl:hasOBONamespace>
        <oboInOwl:id>GAZ:00062915</oboInOwl:id>
        <rdfs:label>Pucioasa</rdfs:label>
    </owl:NamedIndividual>
    


    <!-- http://purl.obolibrary.org/obo/GAZ_00062916 -->

    <owl:NamedIndividual rdf:about="http://purl.obolibrary.org/obo/GAZ_00062916">
        <obo:RO_0001025 rdf:resource="http://purl.obolibrary.org/obo/GAZ_00061983"/>
        <obo:IAO_0000115>A lake in the Ialomita River basin, Romania.</obo:IAO_0000115>
        <oboInOwl:hasOBONamespace>GAZ</oboInOwl:hasOBONamespace>
        <oboInOwl:id>GAZ:00062916</oboInOwl:id>
        <rdfs:label>Scropoasa</rdfs:label>
    </owl:NamedIndividual>
    


    <!-- http://purl.obolibrary.org/obo/GAZ_00062917 -->

    <owl:NamedIndividual rdf:about="http://purl.obolibrary.org/obo/GAZ_00062917">
        <obo:RO_0001025 rdf:resource="http://purl.obolibrary.org/obo/GAZ_00061997"/>
        <obo:RO_0001025 rdf:resource="http://purl.obolibrary.org/obo/GAZ_00387021"/>
        <obo:IAO_0000115>A glacial lake in the Raul Targului River basin, Romania.</obo:IAO_0000115>
        <oboInOwl:hasOBONamespace>GAZ</oboInOwl:hasOBONamespace>
        <oboInOwl:id>GAZ:00062917</oboInOwl:id>
        <rdfs:label>Lacul Iezer</rdfs:label>
    </owl:NamedIndividual>
    


    <!-- http://purl.obolibrary.org/obo/GAZ_00062918 -->

    <owl:NamedIndividual rdf:about="http://purl.obolibrary.org/obo/GAZ_00062918">
        <obo:RO_0001025 rdf:resource="http://purl.obolibrary.org/obo/GAZ_00061994"/>
        <obo:IAO_0000115>A glacial lake in the Raul Doamnei River basin, Romania.</obo:IAO_0000115>
        <oboInOwl:hasOBONamespace>GAZ</oboInOwl:hasOBONamespace>
        <oboInOwl:id>GAZ:00062918</oboInOwl:id>
        <rdfs:label>Valea Rea</rdfs:label>
    </owl:NamedIndividual>
    


    <!-- http://purl.obolibrary.org/obo/GAZ_00062919 -->

    <owl:NamedIndividual rdf:about="http://purl.obolibrary.org/obo/GAZ_00062919">
        <obo:RO_0001025 rdf:resource="http://purl.obolibrary.org/obo/GAZ_00061994"/>
        <obo:IAO_0000115>A glacial lake in the Raul Doamnei River basin, Romania.</obo:IAO_0000115>
        <oboInOwl:hasOBONamespace>GAZ</oboInOwl:hasOBONamespace>
        <oboInOwl:id>GAZ:00062919</oboInOwl:id>
        <rdfs:label>Zarna</rdfs:label>
    </owl:NamedIndividual>
    


    <!-- http://purl.obolibrary.org/obo/GAZ_00062920 -->

    <owl:NamedIndividual rdf:about="http://purl.obolibrary.org/obo/GAZ_00062920">
        <obo:RO_0001025 rdf:resource="http://purl.obolibrary.org/obo/GAZ_00061994"/>
        <obo:IAO_0000115>A glacial lake in the Raul Doamnei River basin, Romania.</obo:IAO_0000115>
        <oboInOwl:hasOBONamespace>GAZ</oboInOwl:hasOBONamespace>
        <oboInOwl:id>GAZ:00062920</oboInOwl:id>
        <rdfs:label>Manastirii</rdfs:label>
    </owl:NamedIndividual>
    


    <!-- http://purl.obolibrary.org/obo/GAZ_00062921 -->

    <owl:NamedIndividual rdf:about="http://purl.obolibrary.org/obo/GAZ_00062921">
        <obo:RO_0001025 rdf:resource="http://purl.obolibrary.org/obo/GAZ_00061994"/>
        <obo:IAO_0000115>A glacial lake in the Raul Doamnei River basin, Romania.</obo:IAO_0000115>
        <oboInOwl:hasOBONamespace>GAZ</oboInOwl:hasOBONamespace>
        <oboInOwl:id>GAZ:00062921</oboInOwl:id>
        <rdfs:label>Scarisoara</rdfs:label>
    </owl:NamedIndividual>
    


    <!-- http://purl.obolibrary.org/obo/GAZ_00062922 -->

    <owl:NamedIndividual rdf:about="http://purl.obolibrary.org/obo/GAZ_00062922">
        <obo:RO_0001025 rdf:resource="http://purl.obolibrary.org/obo/GAZ_00061994"/>
        <obo:IAO_0000115>Glacial lakes in the Raul Doamnei River basin, Romania.</obo:IAO_0000115>
        <oboInOwl:hasOBONamespace>GAZ</oboInOwl:hasOBONamespace>
        <oboInOwl:id>GAZ:00062922</oboInOwl:id>
        <rdfs:label>Galbena Lakes</rdfs:label>
    </owl:NamedIndividual>
    


    <!-- http://purl.obolibrary.org/obo/GAZ_00062923 -->

    <owl:NamedIndividual rdf:about="http://purl.obolibrary.org/obo/GAZ_00062923">
        <obo:RO_0001025 rdf:resource="http://purl.obolibrary.org/obo/GAZ_00061994"/>
        <obo:IAO_0000115>A glacial lake in the Raul Doamnei River basin, Romania.</obo:IAO_0000115>
        <oboInOwl:hasOBONamespace>GAZ</oboInOwl:hasOBONamespace>
        <oboInOwl:id>GAZ:00062923</oboInOwl:id>
        <rdfs:label>Hartop II</rdfs:label>
    </owl:NamedIndividual>
    


    <!-- http://purl.obolibrary.org/obo/GAZ_00062924 -->

    <owl:NamedIndividual rdf:about="http://purl.obolibrary.org/obo/GAZ_00062924">
        <obo:RO_0001025 rdf:resource="http://purl.obolibrary.org/obo/GAZ_00061994"/>
        <obo:IAO_0000115>A glacial lake in the Raul Doamnei River basin, Romania.</obo:IAO_0000115>
        <oboInOwl:hasOBONamespace>GAZ</oboInOwl:hasOBONamespace>
        <oboInOwl:id>GAZ:00062924</oboInOwl:id>
        <rdfs:label>Hartop I</rdfs:label>
    </owl:NamedIndividual>
    


    <!-- http://purl.obolibrary.org/obo/GAZ_00062925 -->

    <owl:NamedIndividual rdf:about="http://purl.obolibrary.org/obo/GAZ_00062925">
        <obo:RO_0001025 rdf:resource="http://purl.obolibrary.org/obo/GAZ_00061994"/>
        <obo:IAO_0000115>A glacial lake in the Raul Doamnei River basin, Romania.</obo:IAO_0000115>
        <oboInOwl:hasOBONamespace>GAZ</oboInOwl:hasOBONamespace>
        <oboInOwl:id>GAZ:00062925</oboInOwl:id>
        <rdfs:label>Jgheburoasa</rdfs:label>
    </owl:NamedIndividual>
    


    <!-- http://purl.obolibrary.org/obo/GAZ_00062926 -->

    <owl:NamedIndividual rdf:about="http://purl.obolibrary.org/obo/GAZ_00062926">
        <obo:RO_0001025 rdf:resource="http://purl.obolibrary.org/obo/GAZ_00061994"/>
        <obo:IAO_0000115>A glacial lake in the Raul Doamnei River basin, Romania.</obo:IAO_0000115>
        <oboInOwl:hasOBONamespace>GAZ</oboInOwl:hasOBONamespace>
        <oboInOwl:id>GAZ:00062926</oboInOwl:id>
        <rdfs:label>Hartop V</rdfs:label>
    </owl:NamedIndividual>
    


    <!-- http://purl.obolibrary.org/obo/GAZ_00062927 -->

    <owl:NamedIndividual rdf:about="http://purl.obolibrary.org/obo/GAZ_00062927">
        <obo:RO_0001025 rdf:resource="http://purl.obolibrary.org/obo/GAZ_00061994"/>
        <obo:IAO_0000115>A glacial lake in the Buda River basin, Romania.</obo:IAO_0000115>
        <oboInOwl:hasOBONamespace>GAZ</oboInOwl:hasOBONamespace>
        <oboInOwl:id>GAZ:00062927</oboInOwl:id>
        <rdfs:label>Buda</rdfs:label>
    </owl:NamedIndividual>
    


    <!-- http://purl.obolibrary.org/obo/GAZ_00062928 -->

    <owl:NamedIndividual rdf:about="http://purl.obolibrary.org/obo/GAZ_00062928">
        <obo:RO_0001025 rdf:resource="http://purl.obolibrary.org/obo/GAZ_00061994"/>
        <obo:IAO_0000115>A glacial lake in the Capra River basin, Romania.</obo:IAO_0000115>
        <oboInOwl:hasOBONamespace>GAZ</oboInOwl:hasOBONamespace>
        <oboInOwl:id>GAZ:00062928</oboInOwl:id>
        <rdfs:label>Lacul Capra</rdfs:label>
    </owl:NamedIndividual>
    


    <!-- http://purl.obolibrary.org/obo/GAZ_00062929 -->

    <owl:NamedIndividual rdf:about="http://purl.obolibrary.org/obo/GAZ_00062929">
        <obo:RO_0001025 rdf:resource="http://purl.obolibrary.org/obo/GAZ_00061994"/>
        <obo:IAO_0000115>A lake in the Raul Doamnei River basin, Romania.</obo:IAO_0000115>
        <oboInOwl:hasOBONamespace>GAZ</oboInOwl:hasOBONamespace>
        <oboInOwl:id>GAZ:00062929</oboInOwl:id>
        <rdfs:label>Vasalatu</rdfs:label>
    </owl:NamedIndividual>
    


    <!-- http://purl.obolibrary.org/obo/GAZ_00062930 -->

    <owl:NamedIndividual rdf:about="http://purl.obolibrary.org/obo/GAZ_00062930">
        <obo:RO_0001025 rdf:resource="http://purl.obolibrary.org/obo/GAZ_00061994"/>
        <obo:IAO_0000115>A lake in the Arges River basin, Romania.</obo:IAO_0000115>
        <oboInOwl:hasOBONamespace>GAZ</oboInOwl:hasOBONamespace>
        <oboInOwl:id>GAZ:00062930</oboInOwl:id>
        <rdfs:label>Oiesti</rdfs:label>
    </owl:NamedIndividual>
    


    <!-- http://purl.obolibrary.org/obo/GAZ_00062931 -->

    <owl:NamedIndividual rdf:about="http://purl.obolibrary.org/obo/GAZ_00062931">
        <obo:RO_0001025 rdf:resource="http://purl.obolibrary.org/obo/GAZ_00061994"/>
        <obo:IAO_0000115>A glacial lake in the Capra River basin, Romania.</obo:IAO_0000115>
        <oboInOwl:hasOBONamespace>GAZ</oboInOwl:hasOBONamespace>
        <oboInOwl:id>GAZ:00062931</oboInOwl:id>
        <rdfs:label>Caltun</rdfs:label>
    </owl:NamedIndividual>
    


    <!-- http://purl.obolibrary.org/obo/GAZ_00062932 -->

    <owl:NamedIndividual rdf:about="http://purl.obolibrary.org/obo/GAZ_00062932">
        <obo:RO_0001025 rdf:resource="http://purl.obolibrary.org/obo/GAZ_00061994"/>
        <obo:IAO_0000115>A glacial lake in the Buda River basin, Romania.</obo:IAO_0000115>
        <oboInOwl:hasOBONamespace>GAZ</oboInOwl:hasOBONamespace>
        <oboInOwl:id>GAZ:00062932</oboInOwl:id>
        <rdfs:label>Podu Giurgiului</rdfs:label>
    </owl:NamedIndividual>
    


    <!-- http://purl.obolibrary.org/obo/GAZ_00062933 -->

    <owl:NamedIndividual rdf:about="http://purl.obolibrary.org/obo/GAZ_00062933">
        <obo:RO_0001025 rdf:resource="http://purl.obolibrary.org/obo/GAZ_00061994"/>
        <obo:IAO_0000115>A lake in the Arges River basin, Romania.</obo:IAO_0000115>
        <oboInOwl:hasOBONamespace>GAZ</oboInOwl:hasOBONamespace>
        <oboInOwl:id>GAZ:00062933</oboInOwl:id>
        <rdfs:label>Cumpana</rdfs:label>
    </owl:NamedIndividual>
    


    <!-- http://purl.obolibrary.org/obo/GAZ_00062934 -->

    <owl:NamedIndividual rdf:about="http://purl.obolibrary.org/obo/GAZ_00062934">
        <obo:RO_0001025 rdf:resource="http://purl.obolibrary.org/obo/GAZ_00061994"/>
        <obo:IAO_0000115>A lake in the Buda River basin, Romania.</obo:IAO_0000115>
        <oboInOwl:hasOBONamespace>GAZ</oboInOwl:hasOBONamespace>
        <oboInOwl:id>GAZ:00062934</oboInOwl:id>
        <rdfs:label>Dobroneagu</rdfs:label>
    </owl:NamedIndividual>
    


    <!-- http://purl.obolibrary.org/obo/GAZ_00062935 -->

    <owl:NamedIndividual rdf:about="http://purl.obolibrary.org/obo/GAZ_00062935">
        <obo:RO_0001025 rdf:resource="http://purl.obolibrary.org/obo/GAZ_00061994"/>
        <obo:IAO_0000115>A glacial lake in the Breaza River basin, Romania.</obo:IAO_0000115>
        <oboInOwl:hasOBONamespace>GAZ</oboInOwl:hasOBONamespace>
        <oboInOwl:id>GAZ:00062935</oboInOwl:id>
        <rdfs:label>Urlea</rdfs:label>
    </owl:NamedIndividual>
    


    <!-- http://purl.obolibrary.org/obo/GAZ_00062936 -->

    <owl:NamedIndividual rdf:about="http://purl.obolibrary.org/obo/GAZ_00062936">
        <obo:RO_0001025 rdf:resource="http://purl.obolibrary.org/obo/GAZ_00061994"/>
        <obo:IAO_0000115>A glacial lake in the Arpas River basin, Romania.</obo:IAO_0000115>
        <oboInOwl:hasOBONamespace>GAZ</oboInOwl:hasOBONamespace>
        <oboInOwl:id>GAZ:00062936</oboInOwl:id>
        <rdfs:label>Podragu Mic</rdfs:label>
    </owl:NamedIndividual>
    


    <!-- http://purl.obolibrary.org/obo/GAZ_00062937 -->

    <owl:NamedIndividual rdf:about="http://purl.obolibrary.org/obo/GAZ_00062937">
        <obo:RO_0001025 rdf:resource="http://purl.obolibrary.org/obo/GAZ_00061994"/>
        <obo:IAO_0000115>A glacial lake in the Balea River basin, Romania.</obo:IAO_0000115>
        <oboInOwl:hasOBONamespace>GAZ</oboInOwl:hasOBONamespace>
        <oboInOwl:id>GAZ:00062937</oboInOwl:id>
        <rdfs:label>Doamnei</rdfs:label>
    </owl:NamedIndividual>
    


    <!-- http://purl.obolibrary.org/obo/GAZ_00062938 -->

    <owl:NamedIndividual rdf:about="http://purl.obolibrary.org/obo/GAZ_00062938">
        <obo:RO_0001025 rdf:resource="http://purl.obolibrary.org/obo/GAZ_00061994"/>
        <obo:IAO_0000115>A glacial lake in the Arpas River basin, Romania.</obo:IAO_0000115>
        <oboInOwl:hasOBONamespace>GAZ</oboInOwl:hasOBONamespace>
        <oboInOwl:id>GAZ:00062938</oboInOwl:id>
        <rdfs:label>Podragu Mare</rdfs:label>
    </owl:NamedIndividual>
    


    <!-- http://purl.obolibrary.org/obo/GAZ_00062939 -->

    <owl:NamedIndividual rdf:about="http://purl.obolibrary.org/obo/GAZ_00062939">
        <obo:RO_0001025 rdf:resource="http://purl.obolibrary.org/obo/GAZ_00061994"/>
        <obo:IAO_0000115>A glacial lake in the Arpas River basin, Romania.</obo:IAO_0000115>
        <oboInOwl:hasOBONamespace>GAZ</oboInOwl:hasOBONamespace>
        <oboInOwl:id>GAZ:00062939</oboInOwl:id>
        <rdfs:label>Podragel</rdfs:label>
    </owl:NamedIndividual>
    


    <!-- http://purl.obolibrary.org/obo/GAZ_00062940 -->

    <owl:NamedIndividual rdf:about="http://purl.obolibrary.org/obo/GAZ_00062940">
        <obo:RO_0001025 rdf:resource="http://purl.obolibrary.org/obo/GAZ_00061994"/>
        <obo:IAO_0000115>A glacial lake in the Rau Mare River basin, Romania.</obo:IAO_0000115>
        <oboInOwl:hasOBONamespace>GAZ</oboInOwl:hasOBONamespace>
        <oboInOwl:id>GAZ:00062940</oboInOwl:id>
        <rdfs:label>Lacul Avrig</rdfs:label>
    </owl:NamedIndividual>
    


    <!-- http://purl.obolibrary.org/obo/GAZ_00062941 -->

    <owl:NamedIndividual rdf:about="http://purl.obolibrary.org/obo/GAZ_00062941">
        <obo:RO_0001025 rdf:resource="http://purl.obolibrary.org/obo/GAZ_00061990"/>
        <obo:IAO_0000115>A glacial lake in the Sadu River basin, Romania.</obo:IAO_0000115>
        <oboInOwl:hasOBONamespace>GAZ</oboInOwl:hasOBONamespace>
        <oboInOwl:id>GAZ:00062941</oboInOwl:id>
        <rdfs:label>Sadu V</rdfs:label>
    </owl:NamedIndividual>
    


    <!-- http://purl.obolibrary.org/obo/GAZ_00062942 -->

    <owl:NamedIndividual rdf:about="http://purl.obolibrary.org/obo/GAZ_00062942">
        <obo:RO_0001025 rdf:resource="http://purl.obolibrary.org/obo/GAZ_00061990"/>
        <obo:IAO_0000115>A glacial lake in the Rau Mare River basin, Romania.</obo:IAO_0000115>
        <oboInOwl:hasOBONamespace>GAZ</oboInOwl:hasOBONamespace>
        <oboInOwl:id>GAZ:00062942</oboInOwl:id>
        <rdfs:label>Iezeru Mic</rdfs:label>
    </owl:NamedIndividual>
    


    <!-- http://purl.obolibrary.org/obo/GAZ_00062943 -->

    <owl:NamedIndividual rdf:about="http://purl.obolibrary.org/obo/GAZ_00062943">
        <obo:RO_0001025 rdf:resource="http://purl.obolibrary.org/obo/GAZ_00061990"/>
        <obo:IAO_0000115>A glacial lake in the Rau Mare River basin, Romania.</obo:IAO_0000115>
        <oboInOwl:hasOBONamespace>GAZ</oboInOwl:hasOBONamespace>
        <oboInOwl:id>GAZ:00062943</oboInOwl:id>
        <rdfs:label>Iezeru Mare</rdfs:label>
    </owl:NamedIndividual>
    


    <!-- http://purl.obolibrary.org/obo/GAZ_00062944 -->

    <owl:NamedIndividual rdf:about="http://purl.obolibrary.org/obo/GAZ_00062944">
        <obo:RO_0001025 rdf:resource="http://purl.obolibrary.org/obo/GAZ_00061990"/>
        <obo:IAO_0000115>A lake in the Rau Mare River basin, Romania.</obo:IAO_0000115>
        <oboInOwl:hasOBONamespace>GAZ</oboInOwl:hasOBONamespace>
        <oboInOwl:id>GAZ:00062944</oboInOwl:id>
        <rdfs:label>Gura Raului</rdfs:label>
    </owl:NamedIndividual>
    


    <!-- http://purl.obolibrary.org/obo/GAZ_00062945 -->

    <owl:NamedIndividual rdf:about="http://purl.obolibrary.org/obo/GAZ_00062945">
        <obo:RO_0001025 rdf:resource="http://purl.obolibrary.org/obo/GAZ_00061987"/>
        <obo:IAO_0000115>A reservoir in the Sebes River basin, Romania.</obo:IAO_0000115>
        <oboInOwl:hasOBONamespace>GAZ</oboInOwl:hasOBONamespace>
        <oboInOwl:id>GAZ:00062945</oboInOwl:id>
        <rdfs:label>Barajul Oasa</rdfs:label>
    </owl:NamedIndividual>
    


    <!-- http://purl.obolibrary.org/obo/GAZ_00062946 -->

    <owl:NamedIndividual rdf:about="http://purl.obolibrary.org/obo/GAZ_00062946">
        <obo:RO_0001025 rdf:resource="http://purl.obolibrary.org/obo/GAZ_00061987"/>
        <obo:IAO_0000115>A glacial lake in the Rau Mare River basin, Romania.</obo:IAO_0000115>
        <oboInOwl:hasOBONamespace>GAZ</oboInOwl:hasOBONamespace>
        <oboInOwl:id>GAZ:00062946</oboInOwl:id>
        <rdfs:label>Surianu</rdfs:label>
    </owl:NamedIndividual>
    


    <!-- http://purl.obolibrary.org/obo/GAZ_00062947 -->

    <owl:NamedIndividual rdf:about="http://purl.obolibrary.org/obo/GAZ_00062947">
        <obo:RO_0001025 rdf:resource="http://purl.obolibrary.org/obo/GAZ_00061993"/>
        <obo:IAO_0000115>A glaciallake in the Lotru River basin. Romania.</obo:IAO_0000115>
        <oboInOwl:hasOBONamespace>GAZ</oboInOwl:hasOBONamespace>
        <oboInOwl:id>GAZ:00062947</oboInOwl:id>
        <rdfs:label>Iezer-Latorita</rdfs:label>
    </owl:NamedIndividual>
    


    <!-- http://purl.obolibrary.org/obo/GAZ_00062948 -->

    <owl:NamedIndividual rdf:about="http://purl.obolibrary.org/obo/GAZ_00062948">
        <obo:RO_0001025 rdf:resource="http://purl.obolibrary.org/obo/GAZ_00061993"/>
        <obo:IAO_0000115>A glacial lake in the Jiet River Basin, Romania.</obo:IAO_0000115>
        <oboInOwl:hasOBONamespace>GAZ</oboInOwl:hasOBONamespace>
        <oboInOwl:id>GAZ:00062948</oboInOwl:id>
        <rdfs:label>Mija</rdfs:label>
    </owl:NamedIndividual>
    


    <!-- http://purl.obolibrary.org/obo/GAZ_00062949 -->

    <owl:NamedIndividual rdf:about="http://purl.obolibrary.org/obo/GAZ_00062949">
        <obo:RO_0001025 rdf:resource="http://purl.obolibrary.org/obo/GAZ_00061993"/>
        <obo:IAO_0000115>A glacial lake in the Lotru River basin. Romania.</obo:IAO_0000115>
        <oboInOwl:hasOBONamespace>GAZ</oboInOwl:hasOBONamespace>
        <oboInOwl:id>GAZ:00062949</oboInOwl:id>
        <rdfs:label>Iezer Parang</rdfs:label>
    </owl:NamedIndividual>
    


    <!-- http://purl.obolibrary.org/obo/GAZ_00062950 -->

    <owl:NamedIndividual rdf:about="http://purl.obolibrary.org/obo/GAZ_00062950">
        <obo:RO_0001025 rdf:resource="http://purl.obolibrary.org/obo/GAZ_00061993"/>
        <obo:IAO_0000115>A lake in the Lotru River basin. Romania.</obo:IAO_0000115>
        <oboInOwl:hasOBONamespace>GAZ</oboInOwl:hasOBONamespace>
        <oboInOwl:id>GAZ:00062950</oboInOwl:id>
        <rdfs:label>Petrimanu</rdfs:label>
    </owl:NamedIndividual>
    


    <!-- http://purl.obolibrary.org/obo/GAZ_00062951 -->

    <owl:NamedIndividual rdf:about="http://purl.obolibrary.org/obo/GAZ_00062951">
        <obo:RO_0001025 rdf:resource="http://purl.obolibrary.org/obo/GAZ_00061993"/>
        <obo:IAO_0000115>A lake in the Lotru River basin. Romania.</obo:IAO_0000115>
        <oboInOwl:hasOBONamespace>GAZ</oboInOwl:hasOBONamespace>
        <oboInOwl:id>GAZ:00062951</oboInOwl:id>
        <rdfs:label>Pasari</rdfs:label>
    </owl:NamedIndividual>
    


    <!-- http://purl.obolibrary.org/obo/GAZ_00062952 -->

    <owl:NamedIndividual rdf:about="http://purl.obolibrary.org/obo/GAZ_00062952">
        <obo:RO_0001025 rdf:resource="http://purl.obolibrary.org/obo/GAZ_00061993"/>
        <obo:IAO_0000115>A lake in the Lotru River basin. Romania.</obo:IAO_0000115>
        <oboInOwl:hasOBONamespace>GAZ</oboInOwl:hasOBONamespace>
        <oboInOwl:id>GAZ:00062952</oboInOwl:id>
        <rdfs:label>Balindru</rdfs:label>
    </owl:NamedIndividual>
    


    <!-- http://purl.obolibrary.org/obo/GAZ_00062953 -->

    <owl:NamedIndividual rdf:about="http://purl.obolibrary.org/obo/GAZ_00062953">
        <obo:RO_0001025 rdf:resource="http://purl.obolibrary.org/obo/GAZ_00061993"/>
        <obo:IAO_0000115>A glaciallake in the Lotru River basin. Romania.</obo:IAO_0000115>
        <oboInOwl:hasOBONamespace>GAZ</oboInOwl:hasOBONamespace>
        <oboInOwl:id>GAZ:00062953</oboInOwl:id>
        <rdfs:label>Calcescu I</rdfs:label>
    </owl:NamedIndividual>
    


    <!-- http://purl.obolibrary.org/obo/GAZ_00062954 -->

    <owl:NamedIndividual rdf:about="http://purl.obolibrary.org/obo/GAZ_00062954">
        <obo:RO_0001025 rdf:resource="http://purl.obolibrary.org/obo/GAZ_00061993"/>
        <obo:IAO_0000115>A lake in the Lotru River basin. Romania.</obo:IAO_0000115>
        <oboInOwl:hasOBONamespace>GAZ</oboInOwl:hasOBONamespace>
        <oboInOwl:id>GAZ:00062954</oboInOwl:id>
        <rdfs:label>Malaia</rdfs:label>
    </owl:NamedIndividual>
    


    <!-- http://purl.obolibrary.org/obo/GAZ_00062955 -->

    <owl:NamedIndividual rdf:about="http://purl.obolibrary.org/obo/GAZ_00062955">
        <obo:RO_0001025 rdf:resource="http://purl.obolibrary.org/obo/GAZ_00061993"/>
        <obo:IAO_0000115>A glacial lake in the Lotru River basin. Romania.</obo:IAO_0000115>
        <oboInOwl:hasOBONamespace>GAZ</oboInOwl:hasOBONamespace>
        <oboInOwl:id>GAZ:00062955</oboInOwl:id>
        <rdfs:label>Calcescu</rdfs:label>
    </owl:NamedIndividual>
    


    <!-- http://purl.obolibrary.org/obo/GAZ_00062956 -->

    <owl:NamedIndividual rdf:about="http://purl.obolibrary.org/obo/GAZ_00062956">
        <obo:RO_0001025 rdf:resource="http://purl.obolibrary.org/obo/GAZ_00061993"/>
        <obo:IAO_0000115>A lake in the Lotru River basin. Romania.</obo:IAO_0000115>
        <oboInOwl:hasOBONamespace>GAZ</oboInOwl:hasOBONamespace>
        <oboInOwl:id>GAZ:00062956</oboInOwl:id>
        <rdfs:label>Jidoaia</rdfs:label>
    </owl:NamedIndividual>
    


    <!-- http://purl.obolibrary.org/obo/GAZ_00062957 -->

    <owl:NamedIndividual rdf:about="http://purl.obolibrary.org/obo/GAZ_00062957">
        <obo:RO_0001025 rdf:resource="http://purl.obolibrary.org/obo/GAZ_00061993"/>
        <obo:IAO_0000115>A lake in the Lotru River basin. Romania.</obo:IAO_0000115>
        <oboInOwl:hasOBONamespace>GAZ</oboInOwl:hasOBONamespace>
        <oboInOwl:id>GAZ:00062957</oboInOwl:id>
        <rdfs:label>Galbenu</rdfs:label>
    </owl:NamedIndividual>
    


    <!-- http://purl.obolibrary.org/obo/GAZ_00062958 -->

    <owl:NamedIndividual rdf:about="http://purl.obolibrary.org/obo/GAZ_00062958">
        <obo:RO_0001025 rdf:resource="http://purl.obolibrary.org/obo/GAZ_00061993"/>
        <obo:IAO_0000115>A glacial lake in the Jiet River Basin, Romania.</obo:IAO_0000115>
        <oboInOwl:hasOBONamespace>GAZ</oboInOwl:hasOBONamespace>
        <oboInOwl:id>GAZ:00062958</oboInOwl:id>
        <rdfs:label>Mandra</rdfs:label>
    </owl:NamedIndividual>
    


    <!-- http://purl.obolibrary.org/obo/GAZ_00062959 -->

    <owl:NamedIndividual rdf:about="http://purl.obolibrary.org/obo/GAZ_00062959">
        <obo:RO_0001025 rdf:resource="http://purl.obolibrary.org/obo/GAZ_00061993"/>
        <obo:IAO_0000115>A glacial lake in the Jiet River Basin, Romania.</obo:IAO_0000115>
        <oboInOwl:hasOBONamespace>GAZ</oboInOwl:hasOBONamespace>
        <oboInOwl:id>GAZ:00062959</oboInOwl:id>
        <rdfs:label>Taul Verde I</rdfs:label>
    </owl:NamedIndividual>
    


    <!-- http://purl.obolibrary.org/obo/GAZ_00062960 -->

    <owl:NamedIndividual rdf:about="http://purl.obolibrary.org/obo/GAZ_00062960">
        <obo:RO_0001025 rdf:resource="http://purl.obolibrary.org/obo/GAZ_00061993"/>
        <obo:IAO_0000115>A glacial lake in the Jiet River Basin, Romania.</obo:IAO_0000115>
        <oboInOwl:hasOBONamespace>GAZ</oboInOwl:hasOBONamespace>
        <oboInOwl:id>GAZ:00062960</oboInOwl:id>
        <rdfs:label>Taul fara Fund</rdfs:label>
    </owl:NamedIndividual>
    


    <!-- http://purl.obolibrary.org/obo/GAZ_00062961 -->

    <owl:NamedIndividual rdf:about="http://purl.obolibrary.org/obo/GAZ_00062961">
        <obo:RO_0001025 rdf:resource="http://purl.obolibrary.org/obo/GAZ_00061993"/>
        <obo:IAO_0000115>A glacial lake in the Jiet River Basin, Romania.</obo:IAO_0000115>
        <oboInOwl:hasOBONamespace>GAZ</oboInOwl:hasOBONamespace>
        <oboInOwl:id>GAZ:00062961</oboInOwl:id>
        <rdfs:label>Slivei</rdfs:label>
    </owl:NamedIndividual>
    


    <!-- http://purl.obolibrary.org/obo/GAZ_00062962 -->

    <owl:NamedIndividual rdf:about="http://purl.obolibrary.org/obo/GAZ_00062962">
        <obo:RO_0001025 rdf:resource="http://purl.obolibrary.org/obo/GAZ_00061993"/>
        <obo:IAO_0000115>A glacial lake in the Jiet River Basin, Romania.</obo:IAO_0000115>
        <oboInOwl:hasOBONamespace>GAZ</oboInOwl:hasOBONamespace>
        <oboInOwl:id>GAZ:00062962</oboInOwl:id>
        <rdfs:label>Taul Verde III</rdfs:label>
    </owl:NamedIndividual>
    


    <!-- http://purl.obolibrary.org/obo/GAZ_00062963 -->

    <owl:NamedIndividual rdf:about="http://purl.obolibrary.org/obo/GAZ_00062963">
        <obo:RO_0001025 rdf:resource="http://purl.obolibrary.org/obo/GAZ_00061993"/>
        <obo:IAO_0000115>A glacial lake in the Jiet River Basin, Romania.</obo:IAO_0000115>
        <oboInOwl:hasOBONamespace>GAZ</oboInOwl:hasOBONamespace>
        <oboInOwl:id>GAZ:00062963</oboInOwl:id>
        <rdfs:label>Zanoaga Stanii</rdfs:label>
    </owl:NamedIndividual>
    


    <!-- http://purl.obolibrary.org/obo/GAZ_00062964 -->

    <owl:NamedIndividual rdf:about="http://purl.obolibrary.org/obo/GAZ_00062964">
        <obo:RO_0001025 rdf:resource="http://purl.obolibrary.org/obo/GAZ_00061993"/>
        <obo:IAO_0000115>A glacial lake in the Jiet River Basin, Romania.</obo:IAO_0000115>
        <oboInOwl:hasOBONamespace>GAZ</oboInOwl:hasOBONamespace>
        <oboInOwl:id>GAZ:00062964</oboInOwl:id>
        <rdfs:label>Taul Inghetat</rdfs:label>
    </owl:NamedIndividual>
    


    <!-- http://purl.obolibrary.org/obo/GAZ_00062965 -->

    <owl:NamedIndividual rdf:about="http://purl.obolibrary.org/obo/GAZ_00062965">
        <obo:RO_0001025 rdf:resource="http://purl.obolibrary.org/obo/GAZ_00061993"/>
        <obo:IAO_0000115>A glacial lake in the Jiet River Basin, Romania.</obo:IAO_0000115>
        <oboInOwl:hasOBONamespace>GAZ</oboInOwl:hasOBONamespace>
        <oboInOwl:id>GAZ:00062965</oboInOwl:id>
        <rdfs:label>Gheresu</rdfs:label>
    </owl:NamedIndividual>
    


    <!-- http://purl.obolibrary.org/obo/GAZ_00062966 -->

    <owl:NamedIndividual rdf:about="http://purl.obolibrary.org/obo/GAZ_00062966">
        <obo:RO_0001025 rdf:resource="http://purl.obolibrary.org/obo/GAZ_00062003"/>
        <obo:IAO_0000115>A glacial lake in the Rau Mare River basin, Romania.</obo:IAO_0000115>
        <oboInOwl:hasOBONamespace>GAZ</oboInOwl:hasOBONamespace>
        <oboInOwl:id>GAZ:00062966</oboInOwl:id>
        <rdfs:label>Agatat</rdfs:label>
    </owl:NamedIndividual>
    


    <!-- http://purl.obolibrary.org/obo/GAZ_00062967 -->

    <owl:NamedIndividual rdf:about="http://purl.obolibrary.org/obo/GAZ_00062967">
        <obo:RO_0001025 rdf:resource="http://purl.obolibrary.org/obo/GAZ_00062003"/>
        <obo:IAO_0000115>A glacial lake in the Rau Mare River basin, Romania.</obo:IAO_0000115>
        <oboInOwl:hasOBONamespace>GAZ</oboInOwl:hasOBONamespace>
        <oboInOwl:id>GAZ:00062967</oboInOwl:id>
        <rdfs:label>Peleaga</rdfs:label>
    </owl:NamedIndividual>
    


    <!-- http://purl.obolibrary.org/obo/GAZ_00062968 -->

    <owl:NamedIndividual rdf:about="http://purl.obolibrary.org/obo/GAZ_00062968">
        <obo:RO_0001025 rdf:resource="http://purl.obolibrary.org/obo/GAZ_00062003"/>
        <obo:IAO_0000115>A glacial lake in the Rau Mare River basin, Romania.</obo:IAO_0000115>
        <oboInOwl:hasOBONamespace>GAZ</oboInOwl:hasOBONamespace>
        <oboInOwl:id>GAZ:00062968</oboInOwl:id>
        <rdfs:label>Ascuns</rdfs:label>
    </owl:NamedIndividual>
    


    <!-- http://purl.obolibrary.org/obo/GAZ_00062969 -->

    <owl:NamedIndividual rdf:about="http://purl.obolibrary.org/obo/GAZ_00062969">
        <obo:RO_0001025 rdf:resource="http://purl.obolibrary.org/obo/GAZ_00062003"/>
        <obo:IAO_0000115>A glacial lake in the Rau Mare River basin, Romania.</obo:IAO_0000115>
        <oboInOwl:hasOBONamespace>GAZ</oboInOwl:hasOBONamespace>
        <oboInOwl:id>GAZ:00062969</oboInOwl:id>
        <rdfs:label>Spurcat</rdfs:label>
    </owl:NamedIndividual>
    


    <!-- http://purl.obolibrary.org/obo/GAZ_00062970 -->

    <owl:NamedIndividual rdf:about="http://purl.obolibrary.org/obo/GAZ_00062970">
        <obo:RO_0001025 rdf:resource="http://purl.obolibrary.org/obo/GAZ_00062003"/>
        <obo:IAO_0000115>A glacial lake in the Rau Mare River basin, Romania.</obo:IAO_0000115>
        <oboInOwl:hasOBONamespace>GAZ</oboInOwl:hasOBONamespace>
        <oboInOwl:id>GAZ:00062970</oboInOwl:id>
        <rdfs:label>Carlig 2</rdfs:label>
    </owl:NamedIndividual>
    


    <!-- http://purl.obolibrary.org/obo/GAZ_00062971 -->

    <owl:NamedIndividual rdf:about="http://purl.obolibrary.org/obo/GAZ_00062971">
        <obo:RO_0001025 rdf:resource="http://purl.obolibrary.org/obo/GAZ_00062003"/>
        <obo:IAO_0000115>A glacial lake in the Rau Mare River basin, Romania.</obo:IAO_0000115>
        <oboInOwl:hasOBONamespace>GAZ</oboInOwl:hasOBONamespace>
        <oboInOwl:id>GAZ:00062971</oboInOwl:id>
        <rdfs:label>Zanoaga</rdfs:label>
    </owl:NamedIndividual>
    


    <!-- http://purl.obolibrary.org/obo/GAZ_00062972 -->

    <owl:NamedIndividual rdf:about="http://purl.obolibrary.org/obo/GAZ_00062972">
        <obo:RO_0001025 rdf:resource="http://purl.obolibrary.org/obo/GAZ_00062003"/>
        <obo:IAO_0000115>A glacial lake in the Rau Mare River basin, Romania.</obo:IAO_0000115>
        <oboInOwl:hasOBONamespace>GAZ</oboInOwl:hasOBONamespace>
        <oboInOwl:id>GAZ:00062972</oboInOwl:id>
        <rdfs:label>Carlig 1</rdfs:label>
    </owl:NamedIndividual>
    


    <!-- http://purl.obolibrary.org/obo/GAZ_00062973 -->

    <owl:NamedIndividual rdf:about="http://purl.obolibrary.org/obo/GAZ_00062973">
        <obo:RO_0001025 rdf:resource="http://purl.obolibrary.org/obo/GAZ_00062003"/>
        <obo:IAO_0000115>A glacial lake in the Rau Mare River basin, Romania.</obo:IAO_0000115>
        <oboInOwl:hasOBONamespace>GAZ</oboInOwl:hasOBONamespace>
        <oboInOwl:id>GAZ:00062973</oboInOwl:id>
        <rdfs:label>Negru</rdfs:label>
    </owl:NamedIndividual>
    


    <!-- http://purl.obolibrary.org/obo/GAZ_00062974 -->

    <owl:NamedIndividual rdf:about="http://purl.obolibrary.org/obo/GAZ_00062974">
        <obo:RO_0001025 rdf:resource="http://purl.obolibrary.org/obo/GAZ_00062003"/>
        <obo:IAO_0000115>A glacial lake in the Rau Mare River basin, Romania.</obo:IAO_0000115>
        <oboInOwl:hasOBONamespace>GAZ</oboInOwl:hasOBONamespace>
        <oboInOwl:id>GAZ:00062974</oboInOwl:id>
        <rdfs:label>Portii</rdfs:label>
    </owl:NamedIndividual>
    


    <!-- http://purl.obolibrary.org/obo/GAZ_00062975 -->

    <owl:NamedIndividual rdf:about="http://purl.obolibrary.org/obo/GAZ_00062975">
        <obo:RO_0001025 rdf:resource="http://purl.obolibrary.org/obo/GAZ_00062003"/>
        <obo:IAO_0000115>A glacial lake in the Rau Mare River basin, Romania.</obo:IAO_0000115>
        <oboInOwl:hasOBONamespace>GAZ</oboInOwl:hasOBONamespace>
        <oboInOwl:id>GAZ:00062975</oboInOwl:id>
        <rdfs:label>Urat</rdfs:label>
    </owl:NamedIndividual>
    


    <!-- http://purl.obolibrary.org/obo/GAZ_00062976 -->

    <owl:NamedIndividual rdf:about="http://purl.obolibrary.org/obo/GAZ_00062976">
        <obo:RO_0001025 rdf:resource="http://purl.obolibrary.org/obo/GAZ_00062003"/>
        <obo:IAO_0000115>A glacial lake in the Rau Mare River basin, Romania.</obo:IAO_0000115>
        <oboInOwl:hasOBONamespace>GAZ</oboInOwl:hasOBONamespace>
        <oboInOwl:id>GAZ:00062976</oboInOwl:id>
        <rdfs:label>Lacul Judele</rdfs:label>
    </owl:NamedIndividual>
    


    <!-- http://purl.obolibrary.org/obo/GAZ_00062977 -->

    <owl:NamedIndividual rdf:about="http://purl.obolibrary.org/obo/GAZ_00062977">
        <obo:RO_0001025 rdf:resource="http://purl.obolibrary.org/obo/GAZ_00062003"/>
        <obo:IAO_0000115>A glacial lake in the Rau Mare River basin, Romania.</obo:IAO_0000115>
        <oboInOwl:hasOBONamespace>GAZ</oboInOwl:hasOBONamespace>
        <oboInOwl:id>GAZ:00062977</oboInOwl:id>
        <rdfs:label>Viorica</rdfs:label>
    </owl:NamedIndividual>
    


    <!-- http://purl.obolibrary.org/obo/GAZ_00062978 -->

    <owl:NamedIndividual rdf:about="http://purl.obolibrary.org/obo/GAZ_00062978">
        <obo:RO_0001025 rdf:resource="http://purl.obolibrary.org/obo/GAZ_00062003"/>
        <obo:IAO_0000115>A glacial lake in the Rau Mare River basin, Romania.</obo:IAO_0000115>
        <oboInOwl:hasOBONamespace>GAZ</oboInOwl:hasOBONamespace>
        <oboInOwl:id>GAZ:00062978</oboInOwl:id>
        <rdfs:label>Lia</rdfs:label>
    </owl:NamedIndividual>
    


    <!-- http://purl.obolibrary.org/obo/GAZ_00062979 -->

    <owl:NamedIndividual rdf:about="http://purl.obolibrary.org/obo/GAZ_00062979">
        <obo:RO_0001025 rdf:resource="http://purl.obolibrary.org/obo/GAZ_00062003"/>
        <obo:IAO_0000115>A glacial lake in the Rau Mare River basin, Romania.</obo:IAO_0000115>
        <oboInOwl:hasOBONamespace>GAZ</oboInOwl:hasOBONamespace>
        <oboInOwl:id>GAZ:00062979</oboInOwl:id>
        <rdfs:label>Slavei</rdfs:label>
    </owl:NamedIndividual>
    


    <!-- http://purl.obolibrary.org/obo/GAZ_00062980 -->

    <owl:NamedIndividual rdf:about="http://purl.obolibrary.org/obo/GAZ_00062980">
        <obo:RO_0001025 rdf:resource="http://purl.obolibrary.org/obo/GAZ_00062003"/>
        <obo:IAO_0000115>A glacial lake in the Rau Mare River basin, Romania.</obo:IAO_0000115>
        <oboInOwl:hasOBONamespace>GAZ</oboInOwl:hasOBONamespace>
        <oboInOwl:id>GAZ:00062980</oboInOwl:id>
        <rdfs:label>Peleguta</rdfs:label>
    </owl:NamedIndividual>
    


    <!-- http://purl.obolibrary.org/obo/GAZ_00062981 -->

    <owl:NamedIndividual rdf:about="http://purl.obolibrary.org/obo/GAZ_00062981">
        <obo:RO_0001025 rdf:resource="http://purl.obolibrary.org/obo/GAZ_00062003"/>
        <obo:IAO_0000115>A glacial lake in the Rau Mare River basin, Romania.</obo:IAO_0000115>
        <oboInOwl:hasOBONamespace>GAZ</oboInOwl:hasOBONamespace>
        <oboInOwl:id>GAZ:00062981</oboInOwl:id>
        <rdfs:label>Rasucit</rdfs:label>
    </owl:NamedIndividual>
    


    <!-- http://purl.obolibrary.org/obo/GAZ_00062982 -->

    <owl:NamedIndividual rdf:about="http://purl.obolibrary.org/obo/GAZ_00062982">
        <obo:RO_0001025 rdf:resource="http://purl.obolibrary.org/obo/GAZ_00062003"/>
        <obo:IAO_0000115>A glacial lake in the Rau Mare River basin, Romania.</obo:IAO_0000115>
        <oboInOwl:hasOBONamespace>GAZ</oboInOwl:hasOBONamespace>
        <oboInOwl:id>GAZ:00062982</oboInOwl:id>
        <rdfs:label>Gemenele</rdfs:label>
    </owl:NamedIndividual>
    


    <!-- http://purl.obolibrary.org/obo/GAZ_00062983 -->

    <owl:NamedIndividual rdf:about="http://purl.obolibrary.org/obo/GAZ_00062983">
        <obo:RO_0001025 rdf:resource="http://purl.obolibrary.org/obo/GAZ_00062003"/>
        <obo:IAO_0000115>A glacial lake in the Rau Mare River basin, Romania.</obo:IAO_0000115>
        <oboInOwl:hasOBONamespace>GAZ</oboInOwl:hasOBONamespace>
        <oboInOwl:id>GAZ:00062983</oboInOwl:id>
        <rdfs:label>Ana</rdfs:label>
    </owl:NamedIndividual>
    


    <!-- http://purl.obolibrary.org/obo/GAZ_00062984 -->

    <owl:NamedIndividual rdf:about="http://purl.obolibrary.org/obo/GAZ_00062984">
        <obo:RO_0001025 rdf:resource="http://purl.obolibrary.org/obo/GAZ_00062003"/>
        <obo:IAO_0000115>A glacial lake in the Rau Mare River basin, Romania.</obo:IAO_0000115>
        <oboInOwl:hasOBONamespace>GAZ</oboInOwl:hasOBONamespace>
        <oboInOwl:id>GAZ:00062984</oboInOwl:id>
        <rdfs:label>Florica</rdfs:label>
    </owl:NamedIndividual>
    


    <!-- http://purl.obolibrary.org/obo/GAZ_00062985 -->

    <owl:NamedIndividual rdf:about="http://purl.obolibrary.org/obo/GAZ_00062985">
        <obo:RO_0001025 rdf:resource="http://purl.obolibrary.org/obo/GAZ_00062003"/>
        <obo:IAO_0000115>A glacial lake in the Rau Mare River basin, Romania.</obo:IAO_0000115>
        <oboInOwl:hasOBONamespace>GAZ</oboInOwl:hasOBONamespace>
        <oboInOwl:id>GAZ:00062985</oboInOwl:id>
        <rdfs:label>Stirbului</rdfs:label>
    </owl:NamedIndividual>
    


    <!-- http://purl.obolibrary.org/obo/GAZ_00062986 -->

    <owl:NamedIndividual rdf:about="http://purl.obolibrary.org/obo/GAZ_00062986">
        <obo:RO_0001025 rdf:resource="http://purl.obolibrary.org/obo/GAZ_00062003"/>
        <obo:IAO_0000115>A glacial lake in the Rau Mare River basin, Romania.</obo:IAO_0000115>
        <oboInOwl:hasOBONamespace>GAZ</oboInOwl:hasOBONamespace>
        <oboInOwl:id>GAZ:00062986</oboInOwl:id>
        <rdfs:label>Steviei</rdfs:label>
    </owl:NamedIndividual>
    


    <!-- http://purl.obolibrary.org/obo/GAZ_00062987 -->

    <owl:NamedIndividual rdf:about="http://purl.obolibrary.org/obo/GAZ_00062987">
        <obo:RO_0001025 rdf:resource="http://purl.obolibrary.org/obo/GAZ_00062003"/>
        <obo:IAO_0000115>A glacial lake in the Rau Mare River basin, Romania.</obo:IAO_0000115>
        <oboInOwl:hasOBONamespace>GAZ</oboInOwl:hasOBONamespace>
        <oboInOwl:id>GAZ:00062987</oboInOwl:id>
        <rdfs:label>Iezilor</rdfs:label>
    </owl:NamedIndividual>
    


    <!-- http://purl.obolibrary.org/obo/GAZ_00062988 -->

    <owl:NamedIndividual rdf:about="http://purl.obolibrary.org/obo/GAZ_00062988">
        <obo:RO_0001025 rdf:resource="http://purl.obolibrary.org/obo/GAZ_00062003"/>
        <obo:IAO_0000115>A glacial lake in the Jiu River basin, Romania.</obo:IAO_0000115>
        <oboInOwl:hasOBONamespace>GAZ</oboInOwl:hasOBONamespace>
        <oboInOwl:id>GAZ:00062988</oboInOwl:id>
        <rdfs:label>Buta</rdfs:label>
    </owl:NamedIndividual>
    


    <!-- http://purl.obolibrary.org/obo/GAZ_00062989 -->

    <owl:NamedIndividual rdf:about="http://purl.obolibrary.org/obo/GAZ_00062989">
        <obo:RO_0001025 rdf:resource="http://purl.obolibrary.org/obo/GAZ_00062003"/>
        <obo:IAO_0000115>A glacial lake in the Rau Barbat River basin, Romania.</obo:IAO_0000115>
        <oboInOwl:hasOBONamespace>GAZ</oboInOwl:hasOBONamespace>
        <oboInOwl:id>GAZ:00062989</oboInOwl:id>
        <rdfs:label>Custura Mare</rdfs:label>
    </owl:NamedIndividual>
    


    <!-- http://purl.obolibrary.org/obo/GAZ_00062990 -->

    <owl:NamedIndividual rdf:about="http://purl.obolibrary.org/obo/GAZ_00062990">
        <obo:RO_0001025 rdf:resource="http://purl.obolibrary.org/obo/GAZ_00062003"/>
        <obo:IAO_0000115>A glacial lake in the Nucsoara River basin, Romania.</obo:IAO_0000115>
        <oboInOwl:hasOBONamespace>GAZ</oboInOwl:hasOBONamespace>
        <oboInOwl:id>GAZ:00062990</oboInOwl:id>
        <rdfs:label>Lacul Galesul</rdfs:label>
    </owl:NamedIndividual>
    


    <!-- http://purl.obolibrary.org/obo/GAZ_00062991 -->

    <owl:NamedIndividual rdf:about="http://purl.obolibrary.org/obo/GAZ_00062991">
        <obo:RO_0001025 rdf:resource="http://purl.obolibrary.org/obo/GAZ_00062003"/>
        <obo:IAO_0000115>A glacial lake in the Rau Barbat River basin, Romania.</obo:IAO_0000115>
        <oboInOwl:hasOBONamespace>GAZ</oboInOwl:hasOBONamespace>
        <oboInOwl:id>GAZ:00062991</oboInOwl:id>
        <rdfs:label>Custura Mica</rdfs:label>
    </owl:NamedIndividual>
    


    <!-- http://purl.obolibrary.org/obo/GAZ_00062992 -->

    <owl:NamedIndividual rdf:about="http://purl.obolibrary.org/obo/GAZ_00062992">
        <obo:RO_0001025 rdf:resource="http://purl.obolibrary.org/obo/GAZ_00062003"/>
        <obo:IAO_0000115>A glacial lake in the Rau Barbat River basin, Romania.</obo:IAO_0000115>
        <oboInOwl:hasOBONamespace>GAZ</oboInOwl:hasOBONamespace>
        <oboInOwl:id>GAZ:00062992</oboInOwl:id>
        <rdfs:label>Tapului</rdfs:label>
    </owl:NamedIndividual>
    


    <!-- http://purl.obolibrary.org/obo/GAZ_00062993 -->

    <owl:NamedIndividual rdf:about="http://purl.obolibrary.org/obo/GAZ_00062993">
        <obo:RO_0001025 rdf:resource="http://purl.obolibrary.org/obo/GAZ_00062003"/>
        <obo:IAO_0000115>A glacial lake in the Rau Barbat River basin, Romania.</obo:IAO_0000115>
        <oboInOwl:hasOBONamespace>GAZ</oboInOwl:hasOBONamespace>
        <oboInOwl:id>GAZ:00062993</oboInOwl:id>
        <rdfs:label>Papusii</rdfs:label>
    </owl:NamedIndividual>
    


    <!-- http://purl.obolibrary.org/obo/GAZ_00062994 -->

    <owl:NamedIndividual rdf:about="http://purl.obolibrary.org/obo/GAZ_00062994">
        <obo:RO_0001025 rdf:resource="http://purl.obolibrary.org/obo/GAZ_00062003"/>
        <obo:IAO_0000115>A glacial lake in the Nucsoara River basin, Romania.</obo:IAO_0000115>
        <oboInOwl:hasOBONamespace>GAZ</oboInOwl:hasOBONamespace>
        <oboInOwl:id>GAZ:00062994</oboInOwl:id>
        <rdfs:label>Valea Rea</rdfs:label>
    </owl:NamedIndividual>
    


    <!-- http://purl.obolibrary.org/obo/GAZ_00062995 -->

    <owl:NamedIndividual rdf:about="http://purl.obolibrary.org/obo/GAZ_00062995">
        <obo:RO_0001025 rdf:resource="http://purl.obolibrary.org/obo/GAZ_00062000"/>
        <obo:IAO_0000115>A glacial lake in the Rau Mare River basin, Romania.</obo:IAO_0000115>
        <oboInOwl:hasOBONamespace>GAZ</oboInOwl:hasOBONamespace>
        <oboInOwl:id>GAZ:00062995</oboInOwl:id>
        <rdfs:label>Gugu</rdfs:label>
    </owl:NamedIndividual>
    


    <!-- http://purl.obolibrary.org/obo/GAZ_00062996 -->

    <owl:NamedIndividual rdf:about="http://purl.obolibrary.org/obo/GAZ_00062996">
        <obo:RO_0001025 rdf:resource="http://purl.obolibrary.org/obo/GAZ_00062000"/>
        <obo:IAO_0000115>A glacial lake in the Rau Mare River basin, Romania.</obo:IAO_0000115>
        <oboInOwl:hasOBONamespace>GAZ</oboInOwl:hasOBONamespace>
        <oboInOwl:id>GAZ:00062996</oboInOwl:id>
        <rdfs:label>Scarisoara</rdfs:label>
    </owl:NamedIndividual>
    


    <!-- http://purl.obolibrary.org/obo/GAZ_00062997 -->

    <owl:NamedIndividual rdf:about="http://purl.obolibrary.org/obo/GAZ_00062997">
        <obo:RO_0001025 rdf:resource="http://purl.obolibrary.org/obo/GAZ_00062000"/>
        <obo:IAO_0000115>A glacial lake in the Rau Mare River basin, Romania.</obo:IAO_0000115>
        <oboInOwl:hasOBONamespace>GAZ</oboInOwl:hasOBONamespace>
        <oboInOwl:id>GAZ:00062997</oboInOwl:id>
        <rdfs:label>Borascu Mare</rdfs:label>
    </owl:NamedIndividual>
    


    <!-- http://purl.obolibrary.org/obo/GAZ_00062998 -->

    <owl:NamedIndividual rdf:about="http://purl.obolibrary.org/obo/GAZ_00062998">
        <obo:RO_0001025 rdf:resource="http://purl.obolibrary.org/obo/GAZ_00062000"/>
        <obo:IAO_0000115>A lake in the Cerna River basin, Romania.</obo:IAO_0000115>
        <oboInOwl:hasOBONamespace>GAZ</oboInOwl:hasOBONamespace>
        <oboInOwl:id>GAZ:00062998</oboInOwl:id>
        <rdfs:label>Valea lui Iovan</rdfs:label>
    </owl:NamedIndividual>
    


    <!-- http://purl.obolibrary.org/obo/GAZ_00062999 -->

    <owl:NamedIndividual rdf:about="http://purl.obolibrary.org/obo/GAZ_00062999">
        <obo:RO_0001025 rdf:resource="http://purl.obolibrary.org/obo/GAZ_00062001"/>
        <obo:IAO_0000115>A lake in the Rau Mare River basin, Romania.</obo:IAO_0000115>
        <oboInOwl:hasOBONamespace>GAZ</oboInOwl:hasOBONamespace>
        <oboInOwl:id>GAZ:00062999</oboInOwl:id>
        <rdfs:label>Netis</rdfs:label>
    </owl:NamedIndividual>
    


    <!-- http://purl.obolibrary.org/obo/GAZ_00063000 -->

    <owl:NamedIndividual rdf:about="http://purl.obolibrary.org/obo/GAZ_00063000">
        <obo:RO_0001025 rdf:resource="http://purl.obolibrary.org/obo/GAZ_00062001"/>
        <obo:IAO_0000115>A lake in the Bistra Ardeal River basin, Romania.</obo:IAO_0000115>
        <oboInOwl:hasOBONamespace>GAZ</oboInOwl:hasOBONamespace>
        <oboInOwl:id>GAZ:00063000</oboInOwl:id>
        <rdfs:label>Bistra</rdfs:label>
    </owl:NamedIndividual>
    


    <!-- http://purl.obolibrary.org/obo/GAZ_00063001 -->

    <owl:NamedIndividual rdf:about="http://purl.obolibrary.org/obo/GAZ_00063001">
        <obo:RO_0001025 rdf:resource="http://purl.obolibrary.org/obo/GAZ_00062004"/>
        <obo:IAO_0000115>A lake in the Jiu de Vest River basin, Romania.</obo:IAO_0000115>
        <oboInOwl:hasOBONamespace>GAZ</oboInOwl:hasOBONamespace>
        <oboInOwl:id>GAZ:00063001</oboInOwl:id>
        <rdfs:label>Tau fara Fund</rdfs:label>
    </owl:NamedIndividual>
    


    <!-- http://purl.obolibrary.org/obo/GAZ_00063002 -->

    <owl:NamedIndividual rdf:about="http://purl.obolibrary.org/obo/GAZ_00063002">
        <obo:RO_0001025 rdf:resource="http://purl.obolibrary.org/obo/GAZ_00062004"/>
        <obo:IAO_0000115>A reservoir in the Jiu de Vest River basin, Romania. Constructed 1967-1973.</obo:IAO_0000115>
        <oboInOwl:hasOBONamespace>GAZ</oboInOwl:hasOBONamespace>
        <oboInOwl:id>GAZ:00063002</oboInOwl:id>
        <rdfs:label>Lacul Valea de Pesti</rdfs:label>
    </owl:NamedIndividual>
    


    <!-- http://purl.obolibrary.org/obo/GAZ_00063003 -->

    <owl:NamedIndividual rdf:about="http://purl.obolibrary.org/obo/GAZ_00063003">
        <obo:RO_0001025 rdf:resource="http://purl.obolibrary.org/obo/GAZ_00062027"/>
        <obo:IAO_0000115>A lake in the Cerna-Mures River basin, Romania.</obo:IAO_0000115>
        <oboInOwl:hasOBONamespace>GAZ</oboInOwl:hasOBONamespace>
        <oboInOwl:id>GAZ:00063003</oboInOwl:id>
        <rdfs:label>Cincis Cerna</rdfs:label>
    </owl:NamedIndividual>
    


    <!-- http://purl.obolibrary.org/obo/GAZ_00063004 -->

    <owl:NamedIndividual rdf:about="http://purl.obolibrary.org/obo/GAZ_00063004">
        <obo:RO_0001025 rdf:resource="http://purl.obolibrary.org/obo/GAZ_00387100"/>
        <obo:IAO_0000115>A storage reservoir in the Caras River basin, Romania.</obo:IAO_0000115>
        <oboInOwl:hasOBONamespace>GAZ</oboInOwl:hasOBONamespace>
        <oboInOwl:id>GAZ:00063004</oboInOwl:id>
        <rdfs:label>Marghitas</rdfs:label>
    </owl:NamedIndividual>
    


    <!-- http://purl.obolibrary.org/obo/GAZ_00063005 -->

    <owl:NamedIndividual rdf:about="http://purl.obolibrary.org/obo/GAZ_00063005">
        <obo:RO_0001025 rdf:resource="http://purl.obolibrary.org/obo/GAZ_00387100"/>
        <obo:IAO_0000115>A storage reservoir in the Barzava River basin, Romania.</obo:IAO_0000115>
        <oboInOwl:hasOBONamespace>GAZ</oboInOwl:hasOBONamespace>
        <oboInOwl:id>GAZ:00063005</oboInOwl:id>
        <rdfs:label>Gozna</rdfs:label>
    </owl:NamedIndividual>
    


    <!-- http://purl.obolibrary.org/obo/GAZ_00063006 -->

    <owl:NamedIndividual rdf:about="http://purl.obolibrary.org/obo/GAZ_00063006">
        <obo:RO_0001025 rdf:resource="http://purl.obolibrary.org/obo/GAZ_00387100"/>
        <obo:IAO_0000115>A reservoir in the Caras River basin, Romania.</obo:IAO_0000115>
        <oboInOwl:hasOBONamespace>GAZ</oboInOwl:hasOBONamespace>
        <oboInOwl:id>GAZ:00063006</oboInOwl:id>
        <rdfs:label>Buhui</rdfs:label>
    </owl:NamedIndividual>
    


    <!-- http://purl.obolibrary.org/obo/GAZ_00063007 -->

    <owl:NamedIndividual rdf:about="http://purl.obolibrary.org/obo/GAZ_00063007">
        <obo:RO_0001025 rdf:resource="http://purl.obolibrary.org/obo/GAZ_00387100"/>
        <obo:IAO_0000115>A storage reservoir in the Timis River basin, Romania.</obo:IAO_0000115>
        <oboInOwl:hasOBONamespace>GAZ</oboInOwl:hasOBONamespace>
        <oboInOwl:id>GAZ:00063007</oboInOwl:id>
        <rdfs:label>Trei Ape</rdfs:label>
    </owl:NamedIndividual>
    


    <!-- http://purl.obolibrary.org/obo/GAZ_00063008 -->

    <owl:NamedIndividual rdf:about="http://purl.obolibrary.org/obo/GAZ_00063008">
        <obo:RO_0001025 rdf:resource="http://purl.obolibrary.org/obo/GAZ_00387100"/>
        <obo:IAO_0000115>A storage reservoir in the Barzava River basin, Romania.</obo:IAO_0000115>
        <oboInOwl:hasOBONamespace>GAZ</oboInOwl:hasOBONamespace>
        <oboInOwl:id>GAZ:00063008</oboInOwl:id>
        <rdfs:label>Secu</rdfs:label>
    </owl:NamedIndividual>
    


    <!-- http://purl.obolibrary.org/obo/GAZ_00063009 -->

    <owl:NamedIndividual rdf:about="http://purl.obolibrary.org/obo/GAZ_00063009">
        <obo:RO_0001025 rdf:resource="http://purl.obolibrary.org/obo/GAZ_00387100"/>
        <obo:IAO_0000115>A storage reservoir in the Barzava River basin, Romania.</obo:IAO_0000115>
        <oboInOwl:hasOBONamespace>GAZ</oboInOwl:hasOBONamespace>
        <oboInOwl:id>GAZ:00063009</oboInOwl:id>
        <rdfs:label>Valiug</rdfs:label>
    </owl:NamedIndividual>
    


    <!-- http://purl.obolibrary.org/obo/GAZ_00063010 -->

    <owl:NamedIndividual rdf:about="http://purl.obolibrary.org/obo/GAZ_00063010">
        <obo:RO_0001025 rdf:resource="http://purl.obolibrary.org/obo/GAZ_00062039"/>
        <obo:IAO_0000115>A storage reservoir in the Caras River basin, Romania.</obo:IAO_0000115>
        <oboInOwl:hasOBONamespace>GAZ</oboInOwl:hasOBONamespace>
        <oboInOwl:id>GAZ:00063010</oboInOwl:id>
        <rdfs:label>Lacu Mic</rdfs:label>
    </owl:NamedIndividual>
    


    <!-- http://purl.obolibrary.org/obo/GAZ_00063011 -->

    <owl:NamedIndividual rdf:about="http://purl.obolibrary.org/obo/GAZ_00063011">
        <obo:RO_0001025 rdf:resource="http://purl.obolibrary.org/obo/GAZ_00062039"/>
        <obo:IAO_0000115>A lake in the Caras River basin, Romania.</obo:IAO_0000115>
        <oboInOwl:hasOBONamespace>GAZ</oboInOwl:hasOBONamespace>
        <oboInOwl:id>GAZ:00063011</oboInOwl:id>
        <rdfs:label>Lacu Mare</rdfs:label>
    </owl:NamedIndividual>
    


    <!-- http://purl.obolibrary.org/obo/GAZ_00063012 -->

    <owl:NamedIndividual rdf:about="http://purl.obolibrary.org/obo/GAZ_00063012">
        <obo:RO_0001025 rdf:resource="http://purl.obolibrary.org/obo/GAZ_00062039"/>
        <obo:IAO_0000115>A storage reservoir in the Barzava River basin, Romania.</obo:IAO_0000115>
        <oboInOwl:hasOBONamespace>GAZ</oboInOwl:hasOBONamespace>
        <oboInOwl:id>GAZ:00063012</oboInOwl:id>
        <rdfs:label>Ferendia</rdfs:label>
    </owl:NamedIndividual>
    


    <!-- http://purl.obolibrary.org/obo/GAZ_00063013 -->

    <owl:NamedIndividual rdf:about="http://purl.obolibrary.org/obo/GAZ_00063013">
        <obo:RO_0001025 rdf:resource="http://purl.obolibrary.org/obo/GAZ_00062038"/>
        <obo:IAO_0000115>A lake in the Caras River basin, Romania.</obo:IAO_0000115>
        <oboInOwl:hasOBONamespace>GAZ</oboInOwl:hasOBONamespace>
        <oboInOwl:id>GAZ:00063013</oboInOwl:id>
        <rdfs:label>Lacu Mic-Oravita</rdfs:label>
    </owl:NamedIndividual>
    


    <!-- http://purl.obolibrary.org/obo/GAZ_00063014 -->

    <owl:NamedIndividual rdf:about="http://purl.obolibrary.org/obo/GAZ_00063014">
        <obo:RO_0001025 rdf:resource="http://purl.obolibrary.org/obo/GAZ_00062038"/>
        <obo:IAO_0000115>A lake in the Caras River basin, Romania.</obo:IAO_0000115>
        <oboInOwl:hasOBONamespace>GAZ</oboInOwl:hasOBONamespace>
        <oboInOwl:id>GAZ:00063014</oboInOwl:id>
        <rdfs:label>Lacu Mare-Oravita</rdfs:label>
    </owl:NamedIndividual>
    


    <!-- http://purl.obolibrary.org/obo/GAZ_00063015 -->

    <owl:NamedIndividual rdf:about="http://purl.obolibrary.org/obo/GAZ_00063015">
        <obo:RO_0001025 rdf:resource="http://purl.obolibrary.org/obo/GAZ_00062025"/>
        <obo:IAO_0000115>A lake in he Ampoi River basin, Romania.</obo:IAO_0000115>
        <oboInOwl:hasOBONamespace>GAZ</oboInOwl:hasOBONamespace>
        <oboInOwl:id>GAZ:00063015</oboInOwl:id>
        <rdfs:label>Iezer Ighiel</rdfs:label>
    </owl:NamedIndividual>
    


    <!-- http://purl.obolibrary.org/obo/GAZ_00063016 -->

    <owl:NamedIndividual rdf:about="http://purl.obolibrary.org/obo/GAZ_00063016">
        <obo:RO_0001025 rdf:resource="http://purl.obolibrary.org/obo/GAZ_00062024"/>
        <obo:IAO_0000115>A lake in the V. Abrudului River basin, Romania.</obo:IAO_0000115>
        <oboInOwl:hasOBONamespace>GAZ</oboInOwl:hasOBONamespace>
        <oboInOwl:id>GAZ:00063016</oboInOwl:id>
        <rdfs:label>Seliste</rdfs:label>
    </owl:NamedIndividual>
    


    <!-- http://purl.obolibrary.org/obo/GAZ_00063017 -->

    <owl:NamedIndividual rdf:about="http://purl.obolibrary.org/obo/GAZ_00063017">
        <obo:RO_0001025 rdf:resource="http://purl.obolibrary.org/obo/GAZ_00062024"/>
        <obo:IAO_0000115>A lake in the V. Abrudului River basin, Romania.</obo:IAO_0000115>
        <oboInOwl:hasOBONamespace>GAZ</oboInOwl:hasOBONamespace>
        <oboInOwl:id>GAZ:00063017</oboInOwl:id>
        <rdfs:label>Tarinii</rdfs:label>
    </owl:NamedIndividual>
    


    <!-- http://purl.obolibrary.org/obo/GAZ_00063018 -->

    <owl:NamedIndividual rdf:about="http://purl.obolibrary.org/obo/GAZ_00063018">
        <obo:RO_0001025 rdf:resource="http://purl.obolibrary.org/obo/GAZ_00062024"/>
        <obo:IAO_0000115>A lake in the Mures River basin, Romania.</obo:IAO_0000115>
        <oboInOwl:hasOBONamespace>GAZ</oboInOwl:hasOBONamespace>
        <oboInOwl:id>GAZ:00063018</oboInOwl:id>
        <rdfs:label>Faerag</rdfs:label>
    </owl:NamedIndividual>
    


    <!-- http://purl.obolibrary.org/obo/GAZ_00063019 -->

    <owl:NamedIndividual rdf:about="http://purl.obolibrary.org/obo/GAZ_00063019">
        <obo:RO_0001025 rdf:resource="http://purl.obolibrary.org/obo/GAZ_00062024"/>
        <obo:IAO_0000115>A lake in the Mures River basin, Romania.</obo:IAO_0000115>
        <oboInOwl:hasOBONamespace>GAZ</oboInOwl:hasOBONamespace>
        <oboInOwl:id>GAZ:00063019</oboInOwl:id>
        <rdfs:label>Caraciu</rdfs:label>
    </owl:NamedIndividual>
    


    <!-- http://purl.obolibrary.org/obo/GAZ_00063020 -->

    <owl:NamedIndividual rdf:about="http://purl.obolibrary.org/obo/GAZ_00063020">
        <obo:RO_0001025 rdf:resource="http://purl.obolibrary.org/obo/GAZ_00062024"/>
        <obo:IAO_0000115>A lake in the V. Abrudului River basin, Romania.</obo:IAO_0000115>
        <oboInOwl:hasOBONamespace>GAZ</oboInOwl:hasOBONamespace>
        <oboInOwl:id>GAZ:00063020</oboInOwl:id>
        <rdfs:label>Corali</rdfs:label>
    </owl:NamedIndividual>
    


    <!-- http://purl.obolibrary.org/obo/GAZ_00063021 -->

    <owl:NamedIndividual rdf:about="http://purl.obolibrary.org/obo/GAZ_00063021">
        <obo:RO_0001025 rdf:resource="http://purl.obolibrary.org/obo/GAZ_00062024"/>
        <obo:IAO_0000115>A lake in the V. Abrudului River basin, Romania.</obo:IAO_0000115>
        <oboInOwl:hasOBONamespace>GAZ</oboInOwl:hasOBONamespace>
        <oboInOwl:id>GAZ:00063021</oboInOwl:id>
        <rdfs:label>Gaurari</rdfs:label>
    </owl:NamedIndividual>
    


    <!-- http://purl.obolibrary.org/obo/GAZ_00063022 -->

    <owl:NamedIndividual rdf:about="http://purl.obolibrary.org/obo/GAZ_00063022">
        <obo:RO_0001025 rdf:resource="http://purl.obolibrary.org/obo/GAZ_00062024"/>
        <obo:IAO_0000115>A lake in the V. Abrudului River basin, Romania.</obo:IAO_0000115>
        <oboInOwl:hasOBONamespace>GAZ</oboInOwl:hasOBONamespace>
        <oboInOwl:id>GAZ:00063022</oboInOwl:id>
        <rdfs:label>Muntari</rdfs:label>
    </owl:NamedIndividual>
    


    <!-- http://purl.obolibrary.org/obo/GAZ_00063023 -->

    <owl:NamedIndividual rdf:about="http://purl.obolibrary.org/obo/GAZ_00063023">
        <obo:RO_0001025 rdf:resource="http://purl.obolibrary.org/obo/GAZ_00062024"/>
        <obo:IAO_0000115>A lake in the V. Abrudului River basin, Romania.</obo:IAO_0000115>
        <oboInOwl:hasOBONamespace>GAZ</oboInOwl:hasOBONamespace>
        <oboInOwl:id>GAZ:00063023</oboInOwl:id>
        <rdfs:label>Lacu Mare</rdfs:label>
    </owl:NamedIndividual>
    


    <!-- http://purl.obolibrary.org/obo/GAZ_00063024 -->

    <owl:NamedIndividual rdf:about="http://purl.obolibrary.org/obo/GAZ_00063024">
        <obo:RO_0001025 rdf:resource="http://purl.obolibrary.org/obo/GAZ_00062024"/>
        <obo:IAO_0000115>A lake in the V. Abrudului River basin, Romania.</obo:IAO_0000115>
        <oboInOwl:hasOBONamespace>GAZ</oboInOwl:hasOBONamespace>
        <oboInOwl:id>GAZ:00063024</oboInOwl:id>
        <rdfs:label>Cartus</rdfs:label>
    </owl:NamedIndividual>
    


    <!-- http://purl.obolibrary.org/obo/GAZ_00063025 -->

    <owl:NamedIndividual rdf:about="http://purl.obolibrary.org/obo/GAZ_00063025">
        <obo:RO_0001025 rdf:resource="http://purl.obolibrary.org/obo/GAZ_00062024"/>
        <obo:IAO_0000115>A lake in the V. Abrudului River basin, Romania.</obo:IAO_0000115>
        <oboInOwl:hasOBONamespace>GAZ</oboInOwl:hasOBONamespace>
        <oboInOwl:id>GAZ:00063025</oboInOwl:id>
        <rdfs:label>Brazi</rdfs:label>
    </owl:NamedIndividual>
    


    <!-- http://purl.obolibrary.org/obo/GAZ_00063026 -->

    <owl:NamedIndividual rdf:about="http://purl.obolibrary.org/obo/GAZ_00063026">
        <obo:RO_0001025 rdf:resource="http://purl.obolibrary.org/obo/GAZ_00062024"/>
        <obo:IAO_0000115>A lake in the V. Abrudului River basin, Romania.</obo:IAO_0000115>
        <oboInOwl:hasOBONamespace>GAZ</oboInOwl:hasOBONamespace>
        <oboInOwl:id>GAZ:00063026</oboInOwl:id>
        <rdfs:label>Anghel</rdfs:label>
    </owl:NamedIndividual>
    


    <!-- http://purl.obolibrary.org/obo/GAZ_00063027 -->

    <owl:NamedIndividual rdf:about="http://purl.obolibrary.org/obo/GAZ_00063027">
        <obo:RO_0001025 rdf:resource="http://purl.obolibrary.org/obo/GAZ_00062020"/>
        <obo:IAO_0000115>A lake in the Crisu Negru River basin, Romania.</obo:IAO_0000115>
        <oboInOwl:hasOBONamespace>GAZ</oboInOwl:hasOBONamespace>
        <oboInOwl:id>GAZ:00063027</oboInOwl:id>
        <rdfs:label>Toplita</rdfs:label>
    </owl:NamedIndividual>
    


    <!-- http://purl.obolibrary.org/obo/GAZ_00063028 -->

    <owl:NamedIndividual rdf:about="http://purl.obolibrary.org/obo/GAZ_00063028">
        <obo:RO_0001025 rdf:resource="http://purl.obolibrary.org/obo/GAZ_00062020"/>
        <obo:IAO_0000115>A lake in the V. Iadului River basin, Romania.</obo:IAO_0000115>
        <oboInOwl:hasOBONamespace>GAZ</oboInOwl:hasOBONamespace>
        <oboInOwl:id>GAZ:00063028</oboInOwl:id>
        <rdfs:label>Lacul Lesu</rdfs:label>
    </owl:NamedIndividual>
    


    <!-- http://purl.obolibrary.org/obo/GAZ_00063029 -->

    <owl:NamedIndividual rdf:about="http://purl.obolibrary.org/obo/GAZ_00063029">
        <obo:RO_0001025 rdf:resource="http://purl.obolibrary.org/obo/GAZ_00062022"/>
        <obo:IAO_0000115>A lake in the Somesu Rece River basin, Romania.</obo:IAO_0000115>
        <oboInOwl:hasOBONamespace>GAZ</oboInOwl:hasOBONamespace>
        <oboInOwl:id>GAZ:00063029</oboInOwl:id>
        <rdfs:label>Izvorul Baii</rdfs:label>
    </owl:NamedIndividual>
    


    <!-- http://purl.obolibrary.org/obo/GAZ_00063030 -->

    <owl:NamedIndividual rdf:about="http://purl.obolibrary.org/obo/GAZ_00063030">
        <obo:RO_0001025 rdf:resource="http://purl.obolibrary.org/obo/GAZ_00062022"/>
        <obo:IAO_0000115>A lake in the Somesu Mic River basin, Romania.</obo:IAO_0000115>
        <oboInOwl:hasOBONamespace>GAZ</oboInOwl:hasOBONamespace>
        <oboInOwl:id>GAZ:00063030</oboInOwl:id>
        <rdfs:label>Gilau</rdfs:label>
    </owl:NamedIndividual>
    


    <!-- http://purl.obolibrary.org/obo/GAZ_00063032 -->

    <owl:NamedIndividual rdf:about="http://purl.obolibrary.org/obo/GAZ_00063032">
        <obo:RO_0001025 rdf:resource="http://purl.obolibrary.org/obo/GAZ_00062022"/>
        <obo:IAO_0000115>A lake in the Somesu Rece River basin, Romania.</obo:IAO_0000115>
        <oboInOwl:hasOBONamespace>GAZ</oboInOwl:hasOBONamespace>
        <oboInOwl:id>GAZ:00063032</oboInOwl:id>
        <rdfs:label>Blajoaia</rdfs:label>
    </owl:NamedIndividual>
    


    <!-- http://purl.obolibrary.org/obo/GAZ_00063033 -->

    <owl:NamedIndividual rdf:about="http://purl.obolibrary.org/obo/GAZ_00063033">
        <obo:RO_0001025 rdf:resource="http://purl.obolibrary.org/obo/GAZ_00062022"/>
        <obo:IAO_0000115>A storage reservoir on Aries River basin, Romania.</obo:IAO_0000115>
        <oboInOwl:hasOBONamespace>GAZ</oboInOwl:hasOBONamespace>
        <oboInOwl:id>GAZ:00063033</oboInOwl:id>
        <rdfs:label>Iara</rdfs:label>
    </owl:NamedIndividual>
    


    <!-- http://purl.obolibrary.org/obo/GAZ_00063034 -->

    <owl:NamedIndividual rdf:about="http://purl.obolibrary.org/obo/GAZ_00063034">
        <obo:RO_0001025 rdf:resource="http://purl.obolibrary.org/obo/GAZ_00062022"/>
        <obo:IAO_0000115>A lake in the Somesu Rece River basin, Romania.</obo:IAO_0000115>
        <oboInOwl:hasOBONamespace>GAZ</oboInOwl:hasOBONamespace>
        <oboInOwl:id>GAZ:00063034</oboInOwl:id>
        <rdfs:label>Negruta</rdfs:label>
    </owl:NamedIndividual>
    


    <!-- http://purl.obolibrary.org/obo/GAZ_00063035 -->

    <owl:NamedIndividual rdf:about="http://purl.obolibrary.org/obo/GAZ_00063035">
        <obo:RO_0001025 rdf:resource="http://purl.obolibrary.org/obo/GAZ_00062022"/>
        <obo:IAO_0000115>A lake in the Somesu Cald River basin, Romania.</obo:IAO_0000115>
        <oboInOwl:hasOBONamespace>GAZ</oboInOwl:hasOBONamespace>
        <oboInOwl:id>GAZ:00063035</oboInOwl:id>
        <rdfs:label>Izvorul Alb</rdfs:label>
    </owl:NamedIndividual>
    


    <!-- http://purl.obolibrary.org/obo/GAZ_00063036 -->

    <owl:NamedIndividual rdf:about="http://purl.obolibrary.org/obo/GAZ_00063036">
        <obo:RO_0001025 rdf:resource="http://purl.obolibrary.org/obo/GAZ_00062022"/>
        <obo:IAO_0000115>A lake in the Somesu Cald River basin, Romania.</obo:IAO_0000115>
        <oboInOwl:hasOBONamespace>GAZ</oboInOwl:hasOBONamespace>
        <oboInOwl:id>GAZ:00063036</oboInOwl:id>
        <rdfs:label>Lacul Tarnita</rdfs:label>
    </owl:NamedIndividual>
    


    <!-- http://purl.obolibrary.org/obo/GAZ_00063037 -->

    <owl:NamedIndividual rdf:about="http://purl.obolibrary.org/obo/GAZ_00063037">
        <obo:RO_0001025 rdf:resource="http://purl.obolibrary.org/obo/GAZ_00062022"/>
        <obo:IAO_0000115>A storage reservoir on Aries River basin, Romania.</obo:IAO_0000115>
        <oboInOwl:hasOBONamespace>GAZ</oboInOwl:hasOBONamespace>
        <oboInOwl:id>GAZ:00063037</oboInOwl:id>
        <rdfs:label>Soimu</rdfs:label>
    </owl:NamedIndividual>
    


    <!-- http://purl.obolibrary.org/obo/GAZ_00063050 -->

    <owl:NamedIndividual rdf:about="http://purl.obolibrary.org/obo/GAZ_00063050">
        <obo:RO_0001025 rdf:resource="http://purl.obolibrary.org/obo/GAZ_00061772"/>
        <obo:IAO_0000115>A protected reserve of land in Lesser Poland, in the heart of Pieniny Mountains. It was created in 1954.</obo:IAO_0000115>
        <oboInOwl:hasOBONamespace>GAZ</oboInOwl:hasOBONamespace>
        <oboInOwl:id>GAZ:00063050</oboInOwl:id>
        <rdfs:label>Pieninski Park Narodowy</rdfs:label>
    </owl:NamedIndividual>
    


    <!-- http://purl.obolibrary.org/obo/GAZ_00063051 -->

    <owl:NamedIndividual rdf:about="http://purl.obolibrary.org/obo/GAZ_00063051">
        <obo:RO_0001025 rdf:resource="http://purl.obolibrary.org/obo/GAZ_00061772"/>
        <obo:IAO_0000115>A national park in northern Slovakia. The park is located in the western Pieniny Mountains on the border with Poland. It lies in the districts of Kezmarok and Stara Lubovna in the Presov Region. The park was founded on 1967-01-16, and its borders were adjusted in 1997.</obo:IAO_0000115>
        <oboInOwl:hasOBONamespace>GAZ</oboInOwl:hasOBONamespace>
        <oboInOwl:id>GAZ:00063051</oboInOwl:id>
        <rdfs:label>Pieninsky narodny park</rdfs:label>
    </owl:NamedIndividual>
    


    <!-- http://purl.obolibrary.org/obo/GAZ_00063052 -->

    <owl:NamedIndividual rdf:about="http://purl.obolibrary.org/obo/GAZ_00063052">
        <rdf:type rdf:resource="http://purl.obolibrary.org/obo/ENVO_00000100"/>
        <obo:RO_0001025 rdf:resource="http://purl.obolibrary.org/obo/GAZ_00063051"/>
        <obo:IAO_0000115>A gorge that runs through the Pieniny Mountains in the south of Poland and the north of Slovakia (as Dunajec is the border river between the two countries in the area).</obo:IAO_0000115>
        <oboInOwl:hasOBONamespace>GAZ</oboInOwl:hasOBONamespace>
        <oboInOwl:id>GAZ:00063052</oboInOwl:id>
        <rdfs:label>Dunajec River Gorge</rdfs:label>
    </owl:NamedIndividual>
    


    <!-- http://purl.obolibrary.org/obo/GAZ_00063097 -->

    <owl:NamedIndividual rdf:about="http://purl.obolibrary.org/obo/GAZ_00063097">
        <obo:RO_0001025 rdf:resource="http://purl.obolibrary.org/obo/GAZ_00061902"/>
        <obo:IAO_0000115>An artificial lake in the Bieszczady Mountains region, more precisely in Lesko County of the Subcarpathian Voivodship of Poland. The lake was created in 1968 by the construction of the Solina Dam on the San River.</obo:IAO_0000115>
        <oboInOwl:hasOBONamespace>GAZ</oboInOwl:hasOBONamespace>
        <oboInOwl:id>GAZ:00063097</oboInOwl:id>
        <rdfs:label>Jezioro Solinskie</rdfs:label>
    </owl:NamedIndividual>
    


    <!-- http://purl.obolibrary.org/obo/GAZ_00088604 -->

    <owl:NamedIndividual rdf:about="http://purl.obolibrary.org/obo/GAZ_00088604">
        <obo:RO_0001025 rdf:resource="http://purl.obolibrary.org/obo/GAZ_00002952"/>
        <obo:IAO_0000115>A national park across the border of Austria and Hungary. One part of its territory belongs to Austria (100 km2) and one part to Hungary (150 km2).</obo:IAO_0000115>
        <oboInOwl:hasOBONamespace>GAZ</oboInOwl:hasOBONamespace>
        <oboInOwl:id>GAZ:00088604</oboInOwl:id>
        <rdfs:label>Nationalpark Neusiedler See - Seewinkel</rdfs:label>
    </owl:NamedIndividual>
    


    <!-- http://purl.obolibrary.org/obo/GAZ_00089823 -->

    <owl:NamedIndividual rdf:about="http://purl.obolibrary.org/obo/GAZ_00089823">
        <obo:RO_0001025 rdf:resource="http://purl.obolibrary.org/obo/GAZ_00002952"/>
        <obo:IAO_0000115>A national park and World Heritage Site. Established 1973.</obo:IAO_0000115>
        <oboInOwl:hasOBONamespace>GAZ</oboInOwl:hasOBONamespace>
        <oboInOwl:id>GAZ:00089823</oboInOwl:id>
        <rdfs:label>Hortobagy National Park</rdfs:label>
    </owl:NamedIndividual>
    


    <!-- http://purl.obolibrary.org/obo/GAZ_00089824 -->

    <owl:NamedIndividual rdf:about="http://purl.obolibrary.org/obo/GAZ_00089824">
        <obo:RO_0001025 rdf:resource="http://purl.obolibrary.org/obo/GAZ_00014333"/>
        <obo:IAO_0000115>A national park located mainly in Bacs-Kiskun county, Hungary. It was created in 1975 and declared a biosphere reserve by the UNESCO. The park covers an area of 570 km2 and stretches across the Little Cumania (Kiskunsag) region of the Great Hungarian Plain.</obo:IAO_0000115>
        <oboInOwl:hasOBONamespace>GAZ</oboInOwl:hasOBONamespace>
        <oboInOwl:id>GAZ:00089824</oboInOwl:id>
        <rdfs:label>Kiskunsag National Park</rdfs:label>
    </owl:NamedIndividual>
    


    <!-- http://purl.obolibrary.org/obo/GAZ_00089825 -->

    <owl:NamedIndividual rdf:about="http://purl.obolibrary.org/obo/GAZ_00089825">
        <obo:RO_0001025 rdf:resource="http://purl.obolibrary.org/obo/GAZ_00089824"/>
        <obo:IAO_0000115>A lake near the town of Izsak.</obo:IAO_0000115>
        <oboInOwl:hasOBONamespace>GAZ</oboInOwl:hasOBONamespace>
        <oboInOwl:id>GAZ:00089825</oboInOwl:id>
        <rdfs:label>Lake Kolon</rdfs:label>
    </owl:NamedIndividual>
    


    <!-- http://purl.obolibrary.org/obo/GAZ_00089826 -->

    <owl:NamedIndividual rdf:about="http://purl.obolibrary.org/obo/GAZ_00089826">
        <obo:RO_0001025 rdf:resource="http://purl.obolibrary.org/obo/GAZ_00089824"/>
        <obo:IAO_0000115>A lake.</obo:IAO_0000115>
        <oboInOwl:hasOBONamespace>GAZ</oboInOwl:hasOBONamespace>
        <oboInOwl:id>GAZ:00089826</oboInOwl:id>
        <rdfs:label>Lake Kunfeher</rdfs:label>
    </owl:NamedIndividual>
    


    <!-- http://purl.obolibrary.org/obo/GAZ_00089827 -->

    <owl:NamedIndividual rdf:about="http://purl.obolibrary.org/obo/GAZ_00089827">
        <obo:RO_0001025 rdf:resource="http://purl.obolibrary.org/obo/GAZ_00089824"/>
        <obo:IAO_0000115>A lake.</obo:IAO_0000115>
        <oboInOwl:hasOBONamespace>GAZ</oboInOwl:hasOBONamespace>
        <oboInOwl:id>GAZ:00089827</oboInOwl:id>
        <rdfs:label>Lake Sos</rdfs:label>
    </owl:NamedIndividual>
    


    <!-- http://purl.obolibrary.org/obo/GAZ_00089828 -->

    <owl:NamedIndividual rdf:about="http://purl.obolibrary.org/obo/GAZ_00089828">
        <obo:RO_0001025 rdf:resource="http://purl.obolibrary.org/obo/GAZ_00002952"/>
        <obo:IAO_0000115>A national park in Northern Hungary, in the Aggtelek karst region. Established in 1985. A World Heritage Site.</obo:IAO_0000115>
        <oboInOwl:hasOBONamespace>GAZ</oboInOwl:hasOBONamespace>
        <oboInOwl:id>GAZ:00089828</oboInOwl:id>
        <rdfs:label>Aggtelek National Park</rdfs:label>
    </owl:NamedIndividual>
    


    <!-- http://purl.obolibrary.org/obo/GAZ_00089829 -->

    <owl:NamedIndividual rdf:about="http://purl.obolibrary.org/obo/GAZ_00089829">
        <obo:RO_0001025 rdf:resource="http://purl.obolibrary.org/obo/GAZ_00014341"/>
        <obo:IAO_0000115>A national Park in North-West Hungary in Gyor-Moson-Sopron county. It was created in 1991.</obo:IAO_0000115>
        <oboInOwl:hasOBONamespace>GAZ</oboInOwl:hasOBONamespace>
        <oboInOwl:id>GAZ:00089829</oboInOwl:id>
        <rdfs:label>Ferto-Hansag National Park</rdfs:label>
    </owl:NamedIndividual>
    


    <!-- http://purl.obolibrary.org/obo/GAZ_00089830 -->

    <owl:NamedIndividual rdf:about="http://purl.obolibrary.org/obo/GAZ_00089830">
        <obo:RO_0001025 rdf:resource="http://purl.obolibrary.org/obo/GAZ_00002952"/>
        <obo:IAO_0000115>A national park located in the south west of Hungary. Established in 1996. The majority of national park sites are located within Danube and Drava floodland areas.</obo:IAO_0000115>
        <oboInOwl:hasOBONamespace>GAZ</oboInOwl:hasOBONamespace>
        <oboInOwl:id>GAZ:00089830</oboInOwl:id>
        <rdfs:label>Danube-Drava National Park</rdfs:label>
    </owl:NamedIndividual>
    


    <!-- http://purl.obolibrary.org/obo/GAZ_00089831 -->

    <owl:NamedIndividual rdf:about="http://purl.obolibrary.org/obo/GAZ_00089831">
        <obo:RO_0001025 rdf:resource="http://purl.obolibrary.org/obo/GAZ_00014330"/>
        <obo:IAO_0000115>A national park located in Bekes county, in the Southern Great Plain. Established 1997.</obo:IAO_0000115>
        <oboInOwl:hasOBONamespace>GAZ</oboInOwl:hasOBONamespace>
        <oboInOwl:id>GAZ:00089831</oboInOwl:id>
        <rdfs:label>Koros-Maros National Park</rdfs:label>
    </owl:NamedIndividual>
    


    <!-- http://purl.obolibrary.org/obo/GAZ_00089832 -->

    <owl:NamedIndividual rdf:about="http://purl.obolibrary.org/obo/GAZ_00089832">
        <obo:RO_0001025 rdf:resource="http://purl.obolibrary.org/obo/GAZ_00089831"/>
        <obo:IAO_0000115>An alkaline lake.</obo:IAO_0000115>
        <oboInOwl:hasOBONamespace>GAZ</oboInOwl:hasOBONamespace>
        <oboInOwl:id>GAZ:00089832</oboInOwl:id>
        <rdfs:label>Lake Feher</rdfs:label>
    </owl:NamedIndividual>
    


    <!-- http://purl.obolibrary.org/obo/GAZ_00089833 -->

    <owl:NamedIndividual rdf:about="http://purl.obolibrary.org/obo/GAZ_00089833">
        <obo:RO_0001025 rdf:resource="http://purl.obolibrary.org/obo/GAZ_00002952"/>
        <obo:IAO_0000115>A national park. Established in 1997.</obo:IAO_0000115>
        <oboInOwl:hasOBONamespace>GAZ</oboInOwl:hasOBONamespace>
        <oboInOwl:id>GAZ:00089833</oboInOwl:id>
        <rdfs:label>Upper Balaton National Park</rdfs:label>
    </owl:NamedIndividual>
    


    <!-- http://purl.obolibrary.org/obo/GAZ_00089834 -->

    <owl:NamedIndividual rdf:about="http://purl.obolibrary.org/obo/GAZ_00089834">
        <obo:RO_0001025 rdf:resource="http://purl.obolibrary.org/obo/GAZ_00002952"/>
        <obo:IAO_0000115>A national park.</obo:IAO_0000115>
        <oboInOwl:hasOBONamespace>GAZ</oboInOwl:hasOBONamespace>
        <oboInOwl:id>GAZ:00089834</oboInOwl:id>
        <rdfs:label>Szatmar-Bereg National Park</rdfs:label>
    </owl:NamedIndividual>
    


    <!-- http://purl.obolibrary.org/obo/GAZ_00089835 -->

    <owl:NamedIndividual rdf:about="http://purl.obolibrary.org/obo/GAZ_00089835">
        <obo:RO_0001025 rdf:resource="http://purl.obolibrary.org/obo/GAZ_00002952"/>
        <obo:IAO_0000115>A national park. Established in 1997.</obo:IAO_0000115>
        <oboInOwl:hasOBONamespace>GAZ</oboInOwl:hasOBONamespace>
        <oboInOwl:id>GAZ:00089835</oboInOwl:id>
        <rdfs:label>Danube-Ipoly National Park</rdfs:label>
    </owl:NamedIndividual>
    


    <!-- http://purl.obolibrary.org/obo/GAZ_00089836 -->

    <owl:NamedIndividual rdf:about="http://purl.obolibrary.org/obo/GAZ_00089836">
        <obo:RO_0001025 rdf:resource="http://purl.obolibrary.org/obo/GAZ_00002952"/>
        <obo:IAO_0000115>A national park. Established in 2002.</obo:IAO_0000115>
        <oboInOwl:hasOBONamespace>GAZ</oboInOwl:hasOBONamespace>
        <oboInOwl:id>GAZ:00089836</oboInOwl:id>
        <rdfs:label>Orseg National Park</rdfs:label>
    </owl:NamedIndividual>
    


    <!-- http://purl.obolibrary.org/obo/GAZ_00089837 -->

    <owl:NamedIndividual rdf:about="http://purl.obolibrary.org/obo/GAZ_00089837">
        <obo:RO_0001025 rdf:resource="http://purl.obolibrary.org/obo/GAZ_00089830"/>
        <obo:IAO_0000115>A unique forest that is found between Szekszard and Baja, in Hungary. This is the only remaining tidal area of the Danube in Hungary. Gemenc is part of the Danube-Drava National Park, and it is a nature reserve.</obo:IAO_0000115>
        <oboInOwl:hasOBONamespace>GAZ</oboInOwl:hasOBONamespace>
        <oboInOwl:id>GAZ:00089837</oboInOwl:id>
        <rdfs:label>Gemenc</rdfs:label>
    </owl:NamedIndividual>
    


    <!-- http://purl.obolibrary.org/obo/GAZ_00100714 -->

    <owl:NamedIndividual rdf:about="http://purl.obolibrary.org/obo/GAZ_00100714">
        <obo:RO_0001025 rdf:resource="http://purl.obolibrary.org/obo/GAZ_00088604"/>
        <obo:IAO_0000115>Die grosste von uber 40 salzhaltigen Lacken im burgenlandischen Seewinkel, wenige km nordostlich von Apetlon gelegen.</obo:IAO_0000115>
        <oboInOwl:hasOBONamespace>GAZ</oboInOwl:hasOBONamespace>
        <oboInOwl:id>GAZ:00100714</oboInOwl:id>
        <rdfs:label>Lange Lacke</rdfs:label>
    </owl:NamedIndividual>
    


    <!-- http://purl.obolibrary.org/obo/GAZ_00103536 -->

    <owl:NamedIndividual rdf:about="http://purl.obolibrary.org/obo/GAZ_00103536">
        <obo:IAO_0000115>A reservoir.</obo:IAO_0000115>
        <oboInOwl:hasOBONamespace>GAZ</oboInOwl:hasOBONamespace>
        <oboInOwl:id>GAZ:00103536</oboInOwl:id>
        <rdfs:label>Stauraum Freudenau</rdfs:label>
    </owl:NamedIndividual>
    


    <!-- http://purl.obolibrary.org/obo/GAZ_00103538 -->

    <owl:NamedIndividual rdf:about="http://purl.obolibrary.org/obo/GAZ_00103538">
        <obo:RO_0001025 rdf:resource="http://purl.obolibrary.org/obo/GAZ_00088604"/>
        <obo:IAO_0000115>Eine Salzlacke im osterreichischen Seewinkel im Burgenland.</obo:IAO_0000115>
        <oboInOwl:hasOBONamespace>GAZ</oboInOwl:hasOBONamespace>
        <oboInOwl:id>GAZ:00103538</oboInOwl:id>
        <rdfs:label>Darscho</rdfs:label>
    </owl:NamedIndividual>
    


    <!-- http://purl.obolibrary.org/obo/GAZ_00103539 -->

    <owl:NamedIndividual rdf:about="http://purl.obolibrary.org/obo/GAZ_00103539">
        <obo:RO_0001025 rdf:resource="http://purl.obolibrary.org/obo/GAZ_00088604"/>
        <obo:IAO_0000115>Eine Salzlacke im osterreichischen Seewinkel ostlich des Neusiedlersees, an der Hottergrenze zwischen Illmitz und Podersdorf am See gelegen.</obo:IAO_0000115>
        <oboInOwl:hasOBONamespace>GAZ</oboInOwl:hasOBONamespace>
        <oboInOwl:id>GAZ:00103539</oboInOwl:id>
        <rdfs:label>Birnbaumlacke</rdfs:label>
    </owl:NamedIndividual>
    


    <!-- http://purl.obolibrary.org/obo/GAZ_00103540 -->

    <owl:NamedIndividual rdf:about="http://purl.obolibrary.org/obo/GAZ_00103540">
        <obo:RO_0001025 rdf:resource="http://purl.obolibrary.org/obo/GAZ_00088604"/>
        <obo:IAO_0000115>A saline lake.</obo:IAO_0000115>
        <oboInOwl:hasOBONamespace>GAZ</oboInOwl:hasOBONamespace>
        <oboInOwl:id>GAZ:00103540</oboInOwl:id>
        <rdfs:label>Fuchslochlacke</rdfs:label>
    </owl:NamedIndividual>
    


    <!-- http://purl.obolibrary.org/obo/GAZ_00103879 -->

    <owl:NamedIndividual rdf:about="http://purl.obolibrary.org/obo/GAZ_00103879">
        <rdf:type rdf:resource="http://purl.obolibrary.org/obo/ENVO_00000856"/>
        <obo:RO_0001025 rdf:resource="http://purl.obolibrary.org/obo/GAZ_00103880"/>
    </owl:NamedIndividual>
    


    <!-- http://purl.obolibrary.org/obo/GAZ_00103880 -->

    <owl:NamedIndividual rdf:about="http://purl.obolibrary.org/obo/GAZ_00103880">
        <rdf:type rdf:resource="http://purl.obolibrary.org/obo/ENVO_00000856"/>
        <obo:RO_0001025 rdf:resource="http://purl.obolibrary.org/obo/GAZ_00014333"/>
        <obo:IAO_0000115>A municipality in Bacs-Kiskun county, in the Southern Great Plain region of southern Hungary.</obo:IAO_0000115>
        <oboInOwl:hasOBONamespace>GAZ</oboInOwl:hasOBONamespace>
        <oboInOwl:id>GAZ:00103880</oboInOwl:id>
        <rdfs:label>Municipality of Agasegyhaza</rdfs:label>
    </owl:NamedIndividual>
    


    <!-- http://purl.obolibrary.org/obo/GAZ_00110166 -->

    <owl:NamedIndividual rdf:about="http://purl.obolibrary.org/obo/GAZ_00110166">
        <rdf:type rdf:resource="http://purl.obolibrary.org/obo/ENVO_00000100"/>
        <obo:IAO_0000115>A gorge on the Danube River. It forms part of the boundary between Serbia and Romania. In the broad sense it encompasses a route of 134 km; in the narrow sense it only encompasses the last barrier on this route, just beyond the Romanian city of Orsova, that contains a hydroelectric dam, with two power stations, Iron Gate I Hydro Power Plant and Iron Gate II Hydro Power Plant. The gorge lies between Romania in the north and Serbia in the south. At this point, the river separates the southern Carpathian Mountains from the northwestern foothills of the Balkan Mountains. Romania side of the gorge constitutes the Iron Gate natural park, on the other bank, in Serbia, is located the Derdap National Park.</obo:IAO_0000115>
        <oboInOwl:hasOBONamespace>GAZ</oboInOwl:hasOBONamespace>
        <oboInOwl:id>GAZ:00110166</oboInOwl:id>
        <rdfs:label>Iron Gate</rdfs:label>
    </owl:NamedIndividual>
    


    <!-- http://purl.obolibrary.org/obo/GAZ_00110167 -->

    <owl:NamedIndividual rdf:about="http://purl.obolibrary.org/obo/GAZ_00110167">
        <obo:RO_0001025 rdf:resource="http://purl.obolibrary.org/obo/GAZ_00110166"/>
        <obo:IAO_0000115>The second gorge in the Iron Gate, 15 km long and narrows to 220 m.</obo:IAO_0000115>
        <oboInOwl:hasOBONamespace>GAZ</oboInOwl:hasOBONamespace>
        <oboInOwl:id>GAZ:00110167</oboInOwl:id>
        <rdfs:label>Gospodin Vir</rdfs:label>
    </owl:NamedIndividual>
    


    <!-- http://purl.obolibrary.org/obo/GAZ_00110168 -->

    <owl:NamedIndividual rdf:about="http://purl.obolibrary.org/obo/GAZ_00110168">
        <obo:RO_0001025 rdf:resource="http://purl.obolibrary.org/obo/GAZ_00110166"/>
        <obo:IAO_0000115>The first narrowing of the Danubethat lies beyond the (Romanian) island of Moldova Veche.</obo:IAO_0000115>
        <oboInOwl:hasOBONamespace>GAZ</oboInOwl:hasOBONamespace>
        <oboInOwl:id>GAZ:00110168</oboInOwl:id>
        <rdfs:label>Golubac Gorge</rdfs:label>
    </owl:NamedIndividual>
    


    <!-- http://purl.obolibrary.org/obo/GAZ_00110169 -->

    <owl:NamedIndividual rdf:about="http://purl.obolibrary.org/obo/GAZ_00110169">
        <rdf:type rdf:resource="http://purl.obolibrary.org/obo/ENVO_00000100"/>
        <obo:RO_0001025 rdf:resource="http://purl.obolibrary.org/obo/GAZ_00110166"/>
        <obo:IAO_0000115>A gorge in the Iron Gate.</obo:IAO_0000115>
        <oboInOwl:hasOBONamespace>GAZ</oboInOwl:hasOBONamespace>
        <oboInOwl:id>GAZ:00110169</oboInOwl:id>
        <rdfs:label>Donji Milanovac</rdfs:label>
    </owl:NamedIndividual>
    


    <!-- http://purl.obolibrary.org/obo/GAZ_00110170 -->

    <owl:NamedIndividual rdf:about="http://purl.obolibrary.org/obo/GAZ_00110170">
        <rdf:type rdf:resource="http://purl.obolibrary.org/obo/ENVO_00000100"/>
        <obo:RO_0001025 rdf:resource="http://purl.obolibrary.org/obo/GAZ_00110166"/>
        <obo:IAO_0000115>A gorge in the Iron Gate, the river here narrows to 150 m and reaches a depth of up to 53 m.</obo:IAO_0000115>
        <oboInOwl:hasOBONamespace>GAZ</oboInOwl:hasOBONamespace>
        <oboInOwl:id>GAZ:00110170</oboInOwl:id>
        <rdfs:label>Great Kazan Gorge</rdfs:label>
    </owl:NamedIndividual>
    


    <!-- http://purl.obolibrary.org/obo/GAZ_00110171 -->

    <owl:NamedIndividual rdf:about="http://purl.obolibrary.org/obo/GAZ_00110171">
        <rdf:type rdf:resource="http://purl.obolibrary.org/obo/ENVO_00000100"/>
        <obo:RO_0001025 rdf:resource="http://purl.obolibrary.org/obo/GAZ_00110166"/>
        <obo:IAO_0000115>A gorge in the Iron Gate.</obo:IAO_0000115>
        <oboInOwl:hasOBONamespace>GAZ</oboInOwl:hasOBONamespace>
        <oboInOwl:id>GAZ:00110171</oboInOwl:id>
        <rdfs:label>Small Kazan Gorge</rdfs:label>
    </owl:NamedIndividual>
    


    <!-- http://purl.obolibrary.org/obo/GAZ_00110172 -->

    <owl:NamedIndividual rdf:about="http://purl.obolibrary.org/obo/GAZ_00110172">
        <obo:IAO_0000115>A former island in the Danube, drowned in the 1970&apos;s as a consequence of the Iron Gate hydroelectric project. The island was about 3 km downstream from Orsova and measured 1.75 by 0.4-0.5 km.</obo:IAO_0000115>
        <oboInOwl:hasOBONamespace>GAZ</oboInOwl:hasOBONamespace>
        <oboInOwl:id>GAZ:00110172</oboInOwl:id>
        <rdfs:label>Insula Ada Kaleh</rdfs:label>
    </owl:NamedIndividual>
    


    <!-- http://purl.obolibrary.org/obo/GAZ_00110174 -->

    <owl:NamedIndividual rdf:about="http://purl.obolibrary.org/obo/GAZ_00110174">
        <obo:RO_0001025 rdf:resource="http://purl.obolibrary.org/obo/GAZ_00110166"/>
        <obo:IAO_0000115>A hydroelectric reservoir. Constructed 1964-1972.</obo:IAO_0000115>
        <oboInOwl:hasOBONamespace>GAZ</oboInOwl:hasOBONamespace>
        <oboInOwl:id>GAZ:00110174</oboInOwl:id>
        <rdfs:label>Derdap</rdfs:label>
    </owl:NamedIndividual>
    


    <!-- http://purl.obolibrary.org/obo/GAZ_00110175 -->

    <owl:NamedIndividual rdf:about="http://purl.obolibrary.org/obo/GAZ_00110175">
        <obo:IAO_0000115>A hydroelectric reservoir. Constructed 1977-1984.</obo:IAO_0000115>
        <oboInOwl:hasOBONamespace>GAZ</oboInOwl:hasOBONamespace>
        <oboInOwl:id>GAZ:00110175</oboInOwl:id>
        <rdfs:label>Derdap II</rdfs:label>
    </owl:NamedIndividual>
    


    <!-- http://purl.obolibrary.org/obo/GAZ_00143922 -->

    <owl:NamedIndividual rdf:about="http://purl.obolibrary.org/obo/GAZ_00143922">
        <obo:IAO_0000115>A river that emerges from the confluence of the Opasnica and Verusa Rivers in the Dinaric Alps of Montenegro, flows 144 km northward and converges with the Piva River near the Bosnian border to form the Drina River.</obo:IAO_0000115>
        <oboInOwl:hasOBONamespace>GAZ</oboInOwl:hasOBONamespace>
        <oboInOwl:id>GAZ:00143922</oboInOwl:id>
        <rdfs:label>Tara</rdfs:label>
    </owl:NamedIndividual>
    


    <!-- http://purl.obolibrary.org/obo/GAZ_00148095 -->

    <owl:NamedIndividual rdf:about="http://purl.obolibrary.org/obo/GAZ_00148095">
        <obo:RO_0001025 rdf:resource="http://purl.obolibrary.org/obo/GAZ_00061868"/>
    </owl:NamedIndividual>
    


    <!-- http://purl.obolibrary.org/obo/GAZ_00148096 -->

    <owl:NamedIndividual rdf:about="http://purl.obolibrary.org/obo/GAZ_00148096"/>
    


    <!-- http://purl.obolibrary.org/obo/GAZ_00148097 -->

    <owl:NamedIndividual rdf:about="http://purl.obolibrary.org/obo/GAZ_00148097"/>
    


    <!-- http://purl.obolibrary.org/obo/GAZ_00148098 -->

    <owl:NamedIndividual rdf:about="http://purl.obolibrary.org/obo/GAZ_00148098"/>
    


    <!-- http://purl.obolibrary.org/obo/GAZ_00148099 -->

    <owl:NamedIndividual rdf:about="http://purl.obolibrary.org/obo/GAZ_00148099"/>
    


    <!-- http://purl.obolibrary.org/obo/GAZ_00148100 -->

    <owl:NamedIndividual rdf:about="http://purl.obolibrary.org/obo/GAZ_00148100"/>
    


    <!-- http://purl.obolibrary.org/obo/GAZ_00148101 -->

    <owl:NamedIndividual rdf:about="http://purl.obolibrary.org/obo/GAZ_00148101"/>
    


    <!-- http://purl.obolibrary.org/obo/GAZ_00148102 -->

    <owl:NamedIndividual rdf:about="http://purl.obolibrary.org/obo/GAZ_00148102"/>
    


    <!-- http://purl.obolibrary.org/obo/GAZ_00148103 -->

    <owl:NamedIndividual rdf:about="http://purl.obolibrary.org/obo/GAZ_00148103"/>
    


    <!-- http://purl.obolibrary.org/obo/GAZ_00148104 -->

    <owl:NamedIndividual rdf:about="http://purl.obolibrary.org/obo/GAZ_00148104"/>
    


    <!-- http://purl.obolibrary.org/obo/GAZ_00148105 -->

    <owl:NamedIndividual rdf:about="http://purl.obolibrary.org/obo/GAZ_00148105"/>
    


    <!-- http://purl.obolibrary.org/obo/GAZ_00148106 -->

    <owl:NamedIndividual rdf:about="http://purl.obolibrary.org/obo/GAZ_00148106"/>
    


    <!-- http://purl.obolibrary.org/obo/GAZ_00148107 -->

    <owl:NamedIndividual rdf:about="http://purl.obolibrary.org/obo/GAZ_00148107"/>
    


    <!-- http://purl.obolibrary.org/obo/GAZ_00148108 -->

    <owl:NamedIndividual rdf:about="http://purl.obolibrary.org/obo/GAZ_00148108"/>
    


    <!-- http://purl.obolibrary.org/obo/GAZ_00148109 -->

    <owl:NamedIndividual rdf:about="http://purl.obolibrary.org/obo/GAZ_00148109"/>
    


    <!-- http://purl.obolibrary.org/obo/GAZ_00148110 -->

    <owl:NamedIndividual rdf:about="http://purl.obolibrary.org/obo/GAZ_00148110"/>
    


    <!-- http://purl.obolibrary.org/obo/GAZ_00148111 -->

    <owl:NamedIndividual rdf:about="http://purl.obolibrary.org/obo/GAZ_00148111"/>
    


    <!-- http://purl.obolibrary.org/obo/GAZ_00148112 -->

    <owl:NamedIndividual rdf:about="http://purl.obolibrary.org/obo/GAZ_00148112"/>
    


    <!-- http://purl.obolibrary.org/obo/GAZ_00148113 -->

    <owl:NamedIndividual rdf:about="http://purl.obolibrary.org/obo/GAZ_00148113"/>
    


    <!-- http://purl.obolibrary.org/obo/GAZ_00148114 -->

    <owl:NamedIndividual rdf:about="http://purl.obolibrary.org/obo/GAZ_00148114"/>
    


    <!-- http://purl.obolibrary.org/obo/GAZ_00148115 -->

    <owl:NamedIndividual rdf:about="http://purl.obolibrary.org/obo/GAZ_00148115"/>
    


    <!-- http://purl.obolibrary.org/obo/GAZ_00148117 -->

    <owl:NamedIndividual rdf:about="http://purl.obolibrary.org/obo/GAZ_00148117"/>
    


    <!-- http://purl.obolibrary.org/obo/GAZ_00148118 -->

    <owl:NamedIndividual rdf:about="http://purl.obolibrary.org/obo/GAZ_00148118"/>
    


    <!-- http://purl.obolibrary.org/obo/GAZ_00148119 -->

    <owl:NamedIndividual rdf:about="http://purl.obolibrary.org/obo/GAZ_00148119"/>
    


    <!-- http://purl.obolibrary.org/obo/GAZ_00148120 -->

    <owl:NamedIndividual rdf:about="http://purl.obolibrary.org/obo/GAZ_00148120"/>
    


    <!-- http://purl.obolibrary.org/obo/GAZ_00148530 -->

    <owl:NamedIndividual rdf:about="http://purl.obolibrary.org/obo/GAZ_00148530">
        <obo:IAO_0000115>An artificial lake in the North West of Bulgaria. It collects the waters of the rivers Ogosta, Burzia and Zlatitsa and is located about 600 m to the south-west of the border of Montana. Completed 1986.</obo:IAO_0000115>
        <oboInOwl:hasOBONamespace>GAZ</oboInOwl:hasOBONamespace>
        <oboInOwl:id>GAZ:00148530</oboInOwl:id>
        <rdfs:label>Ogosta Reservoir</rdfs:label>
    </owl:NamedIndividual>
    


    <!-- http://purl.obolibrary.org/obo/GAZ_00148541 -->

    <owl:NamedIndividual rdf:about="http://purl.obolibrary.org/obo/GAZ_00148541">
        <obo:IAO_0000115>A water reservoir and dam near Moravka, Moravian-Silesian Region, Czech Republic. Constructed 1961-1966.</obo:IAO_0000115>
        <oboInOwl:hasOBONamespace>GAZ</oboInOwl:hasOBONamespace>
        <oboInOwl:id>GAZ:00148541</oboInOwl:id>
        <rdfs:label>Vodni nadrz Moravka</rdfs:label>
    </owl:NamedIndividual>
    


    <!-- http://purl.obolibrary.org/obo/GAZ_00148543 -->

    <owl:NamedIndividual rdf:about="http://purl.obolibrary.org/obo/GAZ_00148543">
        <obo:IAO_0000115>A dam and associated reservoir. Located in the Moravian-Silesian Beskids mountain range, Moravian-Silesian Region, Czech Republic. Constructed 1964-1974.</obo:IAO_0000115>
        <oboInOwl:hasOBONamespace>GAZ</oboInOwl:hasOBONamespace>
        <oboInOwl:id>GAZ:00148543</oboInOwl:id>
        <rdfs:label>Vodni nadrz Sance</rdfs:label>
    </owl:NamedIndividual>
    


    <!-- http://purl.obolibrary.org/obo/GAZ_00148545 -->

    <owl:NamedIndividual rdf:about="http://purl.obolibrary.org/obo/GAZ_00148545">
        <obo:IAO_0000115>A dam.</obo:IAO_0000115>
        <oboInOwl:hasOBONamespace>GAZ</oboInOwl:hasOBONamespace>
        <oboInOwl:id>GAZ:00148545</oboInOwl:id>
        <rdfs:label>Zermanice Dam</rdfs:label>
    </owl:NamedIndividual>
    


    <!-- http://purl.obolibrary.org/obo/GAZ_00148548 -->

    <owl:NamedIndividual rdf:about="http://purl.obolibrary.org/obo/GAZ_00148548">
        <obo:IAO_0000115>A dam and reservoir.</obo:IAO_0000115>
        <oboInOwl:hasOBONamespace>GAZ</oboInOwl:hasOBONamespace>
        <oboInOwl:id>GAZ:00148548</oboInOwl:id>
        <rdfs:label>Nove Mlyny III Dam</rdfs:label>
    </owl:NamedIndividual>
    


    <!-- http://purl.obolibrary.org/obo/GAZ_00148549 -->

    <owl:NamedIndividual rdf:about="http://purl.obolibrary.org/obo/GAZ_00148549">
        <obo:IAO_0000115>A dam.</obo:IAO_0000115>
        <oboInOwl:hasOBONamespace>GAZ</oboInOwl:hasOBONamespace>
        <oboInOwl:id>GAZ:00148549</oboInOwl:id>
        <rdfs:label>Vranovska prehrada</rdfs:label>
    </owl:NamedIndividual>
    


    <!-- http://purl.obolibrary.org/obo/GAZ_00148550 -->

    <owl:NamedIndividual rdf:about="http://purl.obolibrary.org/obo/GAZ_00148550">
        <obo:IAO_0000115>A reservoir.</obo:IAO_0000115>
        <oboInOwl:hasOBONamespace>GAZ</oboInOwl:hasOBONamespace>
        <oboInOwl:id>GAZ:00148550</oboInOwl:id>
        <rdfs:label>Nove Mlyny I Dam</rdfs:label>
    </owl:NamedIndividual>
    


    <!-- http://purl.obolibrary.org/obo/GAZ_00148551 -->

    <owl:NamedIndividual rdf:about="http://purl.obolibrary.org/obo/GAZ_00148551">
        <obo:IAO_0000115>A reservoir.</obo:IAO_0000115>
        <oboInOwl:hasOBONamespace>GAZ</oboInOwl:hasOBONamespace>
        <oboInOwl:id>GAZ:00148551</oboInOwl:id>
        <rdfs:label>Nove Mlyny II Dam</rdfs:label>
    </owl:NamedIndividual>
    


    <!-- http://purl.obolibrary.org/obo/GAZ_00148561 -->

    <owl:NamedIndividual rdf:about="http://purl.obolibrary.org/obo/GAZ_00148561">
        <obo:IAO_0000115>A river.</obo:IAO_0000115>
        <oboInOwl:hasOBONamespace>GAZ</oboInOwl:hasOBONamespace>
        <oboInOwl:id>GAZ:00148561</oboInOwl:id>
        <rdfs:label>Odrava</rdfs:label>
    </owl:NamedIndividual>
    


    <!-- http://purl.obolibrary.org/obo/GAZ_00148563 -->

    <owl:NamedIndividual rdf:about="http://purl.obolibrary.org/obo/GAZ_00148563"/>
    


    <!-- http://purl.obolibrary.org/obo/GAZ_00148564 -->

    <owl:NamedIndividual rdf:about="http://purl.obolibrary.org/obo/GAZ_00148564">
        <obo:RO_0001025 rdf:resource="http://purl.obolibrary.org/obo/GAZ_00148563"/>
        <obo:IAO_0000115>A reservoir and dam.</obo:IAO_0000115>
        <oboInOwl:hasOBONamespace>GAZ</oboInOwl:hasOBONamespace>
        <oboInOwl:id>GAZ:00148564</oboInOwl:id>
        <rdfs:label>Nechranice Dam</rdfs:label>
    </owl:NamedIndividual>
    


    <!-- http://purl.obolibrary.org/obo/GAZ_00148565 -->

    <owl:NamedIndividual rdf:about="http://purl.obolibrary.org/obo/GAZ_00148565">
        <obo:RO_0001025 rdf:resource="http://purl.obolibrary.org/obo/GAZ_00148563"/>
        <obo:IAO_0000115>A reservoir.</obo:IAO_0000115>
        <oboInOwl:hasOBONamespace>GAZ</oboInOwl:hasOBONamespace>
        <oboInOwl:id>GAZ:00148565</oboInOwl:id>
        <rdfs:label>Vodni nadrz Skalka</rdfs:label>
    </owl:NamedIndividual>
    


    <!-- http://purl.obolibrary.org/obo/GAZ_00148570 -->

    <owl:NamedIndividual rdf:about="http://purl.obolibrary.org/obo/GAZ_00148570">
        <obo:IAO_0000115>A dam.</obo:IAO_0000115>
        <oboInOwl:hasOBONamespace>GAZ</oboInOwl:hasOBONamespace>
        <oboInOwl:id>GAZ:00148570</oboInOwl:id>
        <rdfs:label>Vir I prehrada</rdfs:label>
    </owl:NamedIndividual>
    


    <!-- http://purl.obolibrary.org/obo/GAZ_00148571 -->

    <owl:NamedIndividual rdf:about="http://purl.obolibrary.org/obo/GAZ_00148571">
        <obo:IAO_0000115>A dam.</obo:IAO_0000115>
        <oboInOwl:hasOBONamespace>GAZ</oboInOwl:hasOBONamespace>
        <oboInOwl:id>GAZ:00148571</oboInOwl:id>
        <rdfs:label>Brnenska prehrada</rdfs:label>
    </owl:NamedIndividual>
    


    <!-- http://purl.obolibrary.org/obo/GAZ_00175965 -->

    <owl:NamedIndividual rdf:about="http://purl.obolibrary.org/obo/GAZ_00175965">
        <obo:RO_0001025 rdf:resource="http://purl.obolibrary.org/obo/GAZ_00005403"/>
        <obo:IAO_0000115>A protected area situated in the Little Carpathians, part of the Carpathian Mountains, in West Slovakia. The southwestern-most area is Devinska Kobyla in Bratislava, and the northeastern-most area is the Cachtice Carpathians at the town of Nove Mesto nad Vahom and the village of Cachtice in the Trencin Region. Established 1976-05-05.</obo:IAO_0000115>
        <oboInOwl:hasOBONamespace>GAZ</oboInOwl:hasOBONamespace>
        <oboInOwl:id>GAZ:00175965</oboInOwl:id>
        <rdfs:label>Little Carpathians Protected Landscape Area</rdfs:label>
    </owl:NamedIndividual>
    


    <!-- http://purl.obolibrary.org/obo/GAZ_00175966 -->

    <owl:NamedIndividual rdf:about="http://purl.obolibrary.org/obo/GAZ_00175966">
        <obo:RO_0001025 rdf:resource="http://purl.obolibrary.org/obo/GAZ_00005403"/>
        <obo:IAO_0000115>A limestone cave in West Slovakia in the Little Carpathians Mountains. It is located around 2 km southwest of the village of Smolenice.</obo:IAO_0000115>
        <oboInOwl:hasOBONamespace>GAZ</oboInOwl:hasOBONamespace>
        <oboInOwl:id>GAZ:00175966</oboInOwl:id>
        <rdfs:label>Driny Cave</rdfs:label>
    </owl:NamedIndividual>
    


    <!-- http://purl.obolibrary.org/obo/GAZ_00175967 -->

    <owl:NamedIndividual rdf:about="http://purl.obolibrary.org/obo/GAZ_00175967">
        <obo:RO_0001025 rdf:resource="http://purl.obolibrary.org/obo/GAZ_00175965"/>
        <obo:IAO_0000115>A forest in Bratislava, Slovakia, located in the foothills of the Little Carpathians.</obo:IAO_0000115>
        <oboInOwl:hasOBONamespace>GAZ</oboInOwl:hasOBONamespace>
        <oboInOwl:id>GAZ:00175967</oboInOwl:id>
        <rdfs:label>Bratislavsky lesny park</rdfs:label>
    </owl:NamedIndividual>
    


    <!-- http://purl.obolibrary.org/obo/GAZ_00176767 -->

    <owl:NamedIndividual rdf:about="http://purl.obolibrary.org/obo/GAZ_00176767">
        <obo:RO_0001025 rdf:resource="http://purl.obolibrary.org/obo/GAZ_00061804"/>
        <obo:RO_0001025 rdf:resource="http://purl.obolibrary.org/obo/GAZ_00061807"/>
        <obo:IAO_0000115>An ice cave in Slovakia, near the mining town of Dobsinska in the Slovak Paradise.</obo:IAO_0000115>
        <oboInOwl:hasOBONamespace>GAZ</oboInOwl:hasOBONamespace>
        <oboInOwl:id>GAZ:00176767</oboInOwl:id>
        <rdfs:label>Dobsinska Ice Cave</rdfs:label>
    </owl:NamedIndividual>
    


    <!-- http://purl.obolibrary.org/obo/GAZ_00176768 -->

    <owl:NamedIndividual rdf:about="http://purl.obolibrary.org/obo/GAZ_00176768">
        <obo:RO_0001025 rdf:resource="http://purl.obolibrary.org/obo/GAZ_00061804"/>
        <obo:RO_0001025 rdf:resource="http://purl.obolibrary.org/obo/GAZ_00089828"/>
        <obo:IAO_0000115>A cave that is partly in Hungary and partly in the Slovak Republic.</obo:IAO_0000115>
        <oboInOwl:hasOBONamespace>GAZ</oboInOwl:hasOBONamespace>
        <oboInOwl:id>GAZ:00176768</oboInOwl:id>
        <rdfs:label>Baradla Cave</rdfs:label>
    </owl:NamedIndividual>
    


    <!-- http://purl.obolibrary.org/obo/GAZ_00176769 -->

    <owl:NamedIndividual rdf:about="http://purl.obolibrary.org/obo/GAZ_00176769">
        <obo:RO_0001025 rdf:resource="http://purl.obolibrary.org/obo/GAZ_00061804"/>
        <obo:IAO_0000115>A stalactite and stalagmite cave in the Slovak Karst, Slovakia.</obo:IAO_0000115>
        <oboInOwl:hasOBONamespace>GAZ</oboInOwl:hasOBONamespace>
        <oboInOwl:id>GAZ:00176769</oboInOwl:id>
        <rdfs:label>Gombasek Cave</rdfs:label>
    </owl:NamedIndividual>
    


    <!-- http://purl.obolibrary.org/obo/GAZ_00178622 -->

    <owl:NamedIndividual rdf:about="http://purl.obolibrary.org/obo/GAZ_00178622">
        <obo:IAO_0000115>A large barrage project on river Danube. Only a part of the project has been finished - under the name Gabcikovo Dam/Waterworks.</obo:IAO_0000115>
        <oboInOwl:hasOBONamespace>GAZ</oboInOwl:hasOBONamespace>
        <oboInOwl:id>GAZ:00178622</oboInOwl:id>
        <rdfs:label>Gabcikovo - Nagymaros Dams</rdfs:label>
    </owl:NamedIndividual>
    


    <!-- http://purl.obolibrary.org/obo/GAZ_00178623 -->

    <owl:NamedIndividual rdf:about="http://purl.obolibrary.org/obo/GAZ_00178623">
        <obo:RO_0001025 rdf:resource="http://purl.obolibrary.org/obo/GAZ_00178622"/>
        <oboInOwl:hasOBONamespace>GAZ</oboInOwl:hasOBONamespace>
        <oboInOwl:id>GAZ:00178623</oboInOwl:id>
        <rdfs:label>Gabcikovo Dam/Waterworks</rdfs:label>
    </owl:NamedIndividual>
    


    <!-- http://purl.obolibrary.org/obo/GAZ_00178624 -->

    <owl:NamedIndividual rdf:about="http://purl.obolibrary.org/obo/GAZ_00178624">
        <obo:RO_0001025 rdf:resource="http://purl.obolibrary.org/obo/GAZ_00178622"/>
        <obo:IAO_0000115>A reservoir in the Slovak Republic.</obo:IAO_0000115>
        <oboInOwl:hasOBONamespace>GAZ</oboInOwl:hasOBONamespace>
        <oboInOwl:id>GAZ:00178624</oboInOwl:id>
        <rdfs:label>Cunovo Reservoir</rdfs:label>
    </owl:NamedIndividual>
    


    <!-- http://purl.obolibrary.org/obo/GAZ_00179189 -->

    <owl:NamedIndividual rdf:about="http://purl.obolibrary.org/obo/GAZ_00179189">
        <obo:RO_0001025 rdf:resource="http://purl.obolibrary.org/obo/GAZ_00061821"/>
        <obo:IAO_0000115>A national park in the northern part of the Mala Fatra mountains. Established 1988.</obo:IAO_0000115>
        <oboInOwl:hasOBONamespace>GAZ</oboInOwl:hasOBONamespace>
        <oboInOwl:id>GAZ:00179189</oboInOwl:id>
        <rdfs:label>Mala Fatra National Park</rdfs:label>
    </owl:NamedIndividual>
    


    <!-- http://purl.obolibrary.org/obo/GAZ_00179190 -->

    <owl:NamedIndividual rdf:about="http://purl.obolibrary.org/obo/GAZ_00179190">
        <obo:RO_0001025 rdf:resource="http://purl.obolibrary.org/obo/GAZ_00179189"/>
        <obo:IAO_0000115>A mountain.</obo:IAO_0000115>
        <oboInOwl:hasOBONamespace>GAZ</oboInOwl:hasOBONamespace>
        <oboInOwl:id>GAZ:00179190</oboInOwl:id>
        <rdfs:label>Maly Rozsutec</rdfs:label>
    </owl:NamedIndividual>
    


    <!-- http://purl.obolibrary.org/obo/GAZ_00179191 -->

    <owl:NamedIndividual rdf:about="http://purl.obolibrary.org/obo/GAZ_00179191">
        <obo:RO_0001025 rdf:resource="http://purl.obolibrary.org/obo/GAZ_00179190"/>
        <obo:IAO_0000115>A calcite cave.</obo:IAO_0000115>
        <oboInOwl:hasOBONamespace>GAZ</oboInOwl:hasOBONamespace>
        <oboInOwl:id>GAZ:00179191</oboInOwl:id>
        <rdfs:label>Krystalova jaskyna</rdfs:label>
    </owl:NamedIndividual>
    


    <!-- http://purl.obolibrary.org/obo/GAZ_00179192 -->

    <owl:NamedIndividual rdf:about="http://purl.obolibrary.org/obo/GAZ_00179192">
        <obo:RO_0001025 rdf:resource="http://purl.obolibrary.org/obo/GAZ_00061822"/>
        <obo:IAO_0000115>A National Park in Slovakia. Most of it lies in the southern part of the Zilina Region and a small part in the northern part of Banska Bystrica Region. Established 2002-04-01.</obo:IAO_0000115>
        <oboInOwl:hasOBONamespace>GAZ</oboInOwl:hasOBONamespace>
        <oboInOwl:id>GAZ:00179192</oboInOwl:id>
        <rdfs:label>Velka Fatra National Park</rdfs:label>
    </owl:NamedIndividual>
    


    <!-- http://purl.obolibrary.org/obo/GAZ_00179193 -->

    <owl:NamedIndividual rdf:about="http://purl.obolibrary.org/obo/GAZ_00179193">
        <obo:RO_0001025 rdf:resource="http://purl.obolibrary.org/obo/GAZ_00061807"/>
        <obo:IAO_0000115>A reservoir. Completed 1956.</obo:IAO_0000115>
        <oboInOwl:hasOBONamespace>GAZ</oboInOwl:hasOBONamespace>
        <oboInOwl:id>GAZ:00179193</oboInOwl:id>
        <rdfs:label>Palcmanska Masa</rdfs:label>
    </owl:NamedIndividual>
    


    <!-- http://purl.obolibrary.org/obo/GAZ_00179194 -->

    <owl:NamedIndividual rdf:about="http://purl.obolibrary.org/obo/GAZ_00179194">
        <obo:RO_0001025 rdf:resource="http://purl.obolibrary.org/obo/GAZ_00056821"/>
        <obo:IAO_0000115>A stalactite show cave in the Slovak part of the Tatra mountains. It is located above the settlement of Tatranske Kotlina.</obo:IAO_0000115>
        <oboInOwl:hasOBONamespace>GAZ</oboInOwl:hasOBONamespace>
        <oboInOwl:id>GAZ:00179194</oboInOwl:id>
        <rdfs:label>Belianska Cave</rdfs:label>
    </owl:NamedIndividual>
    


    <!-- http://purl.obolibrary.org/obo/GAZ_00179195 -->

    <owl:NamedIndividual rdf:about="http://purl.obolibrary.org/obo/GAZ_00179195">
        <obo:RO_0001025 rdf:resource="http://purl.obolibrary.org/obo/GAZ_00007976"/>
        <obo:IAO_0000115>A karst cave in Low Tatras in Slovakia. Located on the northern side of the Low Tatras in the Demanovska Valley between Liptovsky Mikulas and known ski resort Jasna.</obo:IAO_0000115>
        <oboInOwl:hasOBONamespace>GAZ</oboInOwl:hasOBONamespace>
        <oboInOwl:id>GAZ:00179195</oboInOwl:id>
        <rdfs:label>Demanovska Cave of Liberty</rdfs:label>
    </owl:NamedIndividual>
    


    <!-- http://purl.obolibrary.org/obo/GAZ_00179196 -->

    <owl:NamedIndividual rdf:about="http://purl.obolibrary.org/obo/GAZ_00179196">
        <obo:RO_0001025 rdf:resource="http://purl.obolibrary.org/obo/GAZ_00061823"/>
        <obo:RO_0001025 rdf:resource="http://purl.obolibrary.org/obo/GAZ_00061873"/>
        <obo:IAO_0000115>A stalactite cave in Central Slovakia. It is located in the Stare Hory and Kremnica mountain ranges and close to the Velka Fatra mountains. The closest villages are Harmanec and Dolny Harmanec; Banska Bystrica is around 16 km south east of the cave.</obo:IAO_0000115>
        <oboInOwl:hasOBONamespace>GAZ</oboInOwl:hasOBONamespace>
        <oboInOwl:id>GAZ:00179196</oboInOwl:id>
        <rdfs:label>Harmanecka Cave</rdfs:label>
    </owl:NamedIndividual>
    


    <!-- http://purl.obolibrary.org/obo/GAZ_00179197 -->

    <owl:NamedIndividual rdf:about="http://purl.obolibrary.org/obo/GAZ_00179197">
        <obo:RO_0001025 rdf:resource="http://purl.obolibrary.org/obo/GAZ_00007973"/>
        <obo:IAO_0000115>A stalactite show cave near the village of Vazec in northern Slovakia. It lies at an altitude of 748 mtres, in the Liptov Basin near the Biely Vah River, on the northern edge of the Low Tatra mountain range.</obo:IAO_0000115>
        <oboInOwl:hasOBONamespace>GAZ</oboInOwl:hasOBONamespace>
        <oboInOwl:id>GAZ:00179197</oboInOwl:id>
        <rdfs:label>Vazecka Cave</rdfs:label>
    </owl:NamedIndividual>
    


    <!-- http://purl.obolibrary.org/obo/GAZ_00179198 -->

    <owl:NamedIndividual rdf:about="http://purl.obolibrary.org/obo/GAZ_00179198">
        <obo:RO_0001025 rdf:resource="http://purl.obolibrary.org/obo/GAZ_00007973"/>
        <obo:IAO_0000115>A cave of the Upper Hron River Valley.</obo:IAO_0000115>
        <oboInOwl:hasOBONamespace>GAZ</oboInOwl:hasOBONamespace>
        <oboInOwl:id>GAZ:00179198</oboInOwl:id>
        <rdfs:label>Bystrianska Cave</rdfs:label>
    </owl:NamedIndividual>
    


    <!-- http://purl.obolibrary.org/obo/GAZ_00179200 -->

    <owl:NamedIndividual rdf:about="http://purl.obolibrary.org/obo/GAZ_00179200">
        <obo:RO_0001025 rdf:resource="http://purl.obolibrary.org/obo/GAZ_00179198"/>
        <obo:IAO_0000115>A show cave located in the central part of the Low Tatra in high-mountain karst of Dumbier.</obo:IAO_0000115>
        <oboInOwl:hasOBONamespace>GAZ</oboInOwl:hasOBONamespace>
        <oboInOwl:id>GAZ:00179200</oboInOwl:id>
        <rdfs:label>Dead Bats Cave</rdfs:label>
    </owl:NamedIndividual>
    


    <!-- http://purl.obolibrary.org/obo/GAZ_00179201 -->

    <owl:NamedIndividual rdf:about="http://purl.obolibrary.org/obo/GAZ_00179201">
        <obo:RO_0001025 rdf:resource="http://purl.obolibrary.org/obo/GAZ_00061856"/>
        <obo:IAO_0000115>A show cave. A karst cave.</obo:IAO_0000115>
        <oboInOwl:hasOBONamespace>GAZ</oboInOwl:hasOBONamespace>
        <oboInOwl:id>GAZ:00179201</oboInOwl:id>
        <rdfs:label>Bad Hole Cave</rdfs:label>
    </owl:NamedIndividual>
    


    <!-- http://purl.obolibrary.org/obo/GAZ_00179202 -->

    <owl:NamedIndividual rdf:about="http://purl.obolibrary.org/obo/GAZ_00179202">
        <obo:RO_0001025 rdf:resource="http://purl.obolibrary.org/obo/GAZ_00178622"/>
        <obo:IAO_0000115>A reservoir.</obo:IAO_0000115>
        <oboInOwl:hasOBONamespace>GAZ</oboInOwl:hasOBONamespace>
        <oboInOwl:id>GAZ:00179202</oboInOwl:id>
        <rdfs:label>Gabcikovo Reservoir</rdfs:label>
    </owl:NamedIndividual>
    


    <!-- http://purl.obolibrary.org/obo/GAZ_00179203 -->

    <owl:NamedIndividual rdf:about="http://purl.obolibrary.org/obo/GAZ_00179203">
        <obo:RO_0001025 rdf:resource="http://purl.obolibrary.org/obo/GAZ_00179202"/>
        <obo:IAO_0000115>A part of Gabcikovo Teservoir.</obo:IAO_0000115>
        <oboInOwl:hasOBONamespace>GAZ</oboInOwl:hasOBONamespace>
        <oboInOwl:id>GAZ:00179203</oboInOwl:id>
        <rdfs:label>Hrusovska zdrz</rdfs:label>
    </owl:NamedIndividual>
    


    <!-- http://purl.obolibrary.org/obo/GAZ_00179204 -->

    <owl:NamedIndividual rdf:about="http://purl.obolibrary.org/obo/GAZ_00179204">
        <obo:RO_0001025 rdf:resource="http://purl.obolibrary.org/obo/GAZ_00179203"/>
        <obo:IAO_0000115>An artificial island.</obo:IAO_0000115>
        <oboInOwl:hasOBONamespace>GAZ</oboInOwl:hasOBONamespace>
        <oboInOwl:id>GAZ:00179204</oboInOwl:id>
        <rdfs:label>Vtaci ostrov</rdfs:label>
    </owl:NamedIndividual>
    


    <!-- http://purl.obolibrary.org/obo/GAZ_00179205 -->

    <owl:NamedIndividual rdf:about="http://purl.obolibrary.org/obo/GAZ_00179205">
        <obo:RO_0001025 rdf:resource="http://purl.obolibrary.org/obo/GAZ_00061742"/>
        <obo:IAO_0000115>A protected area in the Slovak part of the White Carpathians, part of the Carpathian Mountains, in West Slovakia. The area stretches from Skalica District in the south west to the Puchov District in the north east, folllowing the border between Slovakia and the Czech Republic. Established 1979-07-12.</obo:IAO_0000115>
        <oboInOwl:hasOBONamespace>GAZ</oboInOwl:hasOBONamespace>
        <oboInOwl:id>GAZ:00179205</oboInOwl:id>
        <rdfs:label>Chranena krajinna oblast Bile Karpaty</rdfs:label>
    </owl:NamedIndividual>
    


    <!-- http://purl.obolibrary.org/obo/GAZ_00179206 -->

    <owl:NamedIndividual rdf:about="http://purl.obolibrary.org/obo/GAZ_00179206">
        <obo:RO_0001025 rdf:resource="http://purl.obolibrary.org/obo/GAZ_00061894"/>
        <obo:IAO_0000115>A protected area situated in the Cerova vrchovina Mountains, part of the Western Carpathians, in southern Slovakia. It is situated in the Rimavska Sobota, Poltar and Lucenec districts and ends at the Slovak-Hungary borders in the east. Established 1989-10-10.</obo:IAO_0000115>
        <oboInOwl:hasOBONamespace>GAZ</oboInOwl:hasOBONamespace>
        <oboInOwl:id>GAZ:00179206</oboInOwl:id>
        <rdfs:label>Cerova vrchovina Protected Landscape Area</rdfs:label>
    </owl:NamedIndividual>
    


    <!-- http://purl.obolibrary.org/obo/GAZ_00179209 -->

    <owl:NamedIndividual rdf:about="http://purl.obolibrary.org/obo/GAZ_00179209">
        <obo:RO_0001025 rdf:resource="http://purl.obolibrary.org/obo/GAZ_00061872"/>
        <obo:IAO_0000115>A protected area situated in the Polana Mountains, part of the Slovenske stredohorie Mountains, in Central Slovakia. It is situated in the Banska Bystrica, Brezno, Detva, and Zvolen districts. Established 1981-08-12.</obo:IAO_0000115>
        <oboInOwl:hasOBONamespace>GAZ</oboInOwl:hasOBONamespace>
        <oboInOwl:id>GAZ:00179209</oboInOwl:id>
        <rdfs:label>Polana Protected Landscape Area</rdfs:label>
    </owl:NamedIndividual>
    


    <!-- http://purl.obolibrary.org/obo/GAZ_00179210 -->

    <owl:NamedIndividual rdf:about="http://purl.obolibrary.org/obo/GAZ_00179210">
        <obo:RO_0001025 rdf:resource="http://purl.obolibrary.org/obo/GAZ_00061815"/>
        <obo:RO_0001025 rdf:resource="http://purl.obolibrary.org/obo/GAZ_00061857"/>
        <obo:RO_0001025 rdf:resource="http://purl.obolibrary.org/obo/GAZ_00061865"/>
        <obo:IAO_0000115>A protected area situated in the Tribec and Vtacnik mountains, in western Slovakia. It is situated in the Nitra, Zlate Moravce, Zarnovica, Topolcany, Partizanske and Prievidza districts. Established 1985-06-24.</obo:IAO_0000115>
        <oboInOwl:hasOBONamespace>GAZ</oboInOwl:hasOBONamespace>
        <oboInOwl:id>GAZ:00179210</oboInOwl:id>
        <rdfs:label>Ponitrie Protected Landscape Area</rdfs:label>
    </owl:NamedIndividual>
    


    <!-- http://purl.obolibrary.org/obo/GAZ_00179212 -->

    <owl:NamedIndividual rdf:about="http://purl.obolibrary.org/obo/GAZ_00179212">
        <obo:RO_0001025 rdf:resource="http://purl.obolibrary.org/obo/GAZ_00061868"/>
        <obo:IAO_0000115>A protected area situated in the Banska Stiavnica, Zvolen, Ziar nad Hronom, Zarnovica, Levice and Krupina districts. Established 1979-09-22.</obo:IAO_0000115>
        <oboInOwl:hasOBONamespace>GAZ</oboInOwl:hasOBONamespace>
        <oboInOwl:id>GAZ:00179212</oboInOwl:id>
        <rdfs:label>Stiavnicke vrchy Protected Landscape Area</rdfs:label>
    </owl:NamedIndividual>
    


    <!-- http://purl.obolibrary.org/obo/GAZ_00179213 -->

    <owl:NamedIndividual rdf:about="http://purl.obolibrary.org/obo/GAZ_00179213">
        <obo:RO_0001025 rdf:resource="http://purl.obolibrary.org/obo/GAZ_00061955"/>
        <obo:IAO_0000115>A protected area situated in the middle part of the Vihorlatske vrchy mountains, in eastern Slovakia. It is situated in the Humenne, Sobrance and Snina districts. Established 1973-12-28.</obo:IAO_0000115>
        <oboInOwl:hasOBONamespace>GAZ</oboInOwl:hasOBONamespace>
        <oboInOwl:id>GAZ:00179213</oboInOwl:id>
        <rdfs:label>Vihorlat Protected Landscape Area</rdfs:label>
    </owl:NamedIndividual>
    


    <!-- http://purl.obolibrary.org/obo/GAZ_00179220 -->

    <owl:NamedIndividual rdf:about="http://purl.obolibrary.org/obo/GAZ_00179220">
        <obo:RO_0001025 rdf:resource="http://purl.obolibrary.org/obo/GAZ_00063051"/>
        <obo:IAO_0000115>A protected area preserving a karst cave. Established 1979.</obo:IAO_0000115>
        <oboInOwl:hasOBONamespace>GAZ</oboInOwl:hasOBONamespace>
        <oboInOwl:id>GAZ:00179220</oboInOwl:id>
        <rdfs:label>Narodna prirodna pamiatka Aksamitka</rdfs:label>
    </owl:NamedIndividual>
    


    <!-- http://purl.obolibrary.org/obo/GAZ_00179221 -->

    <owl:NamedIndividual rdf:about="http://purl.obolibrary.org/obo/GAZ_00179221">
        <obo:RO_0001025 rdf:resource="http://purl.obolibrary.org/obo/GAZ_00179206"/>
        <obo:IAO_0000115>A protected area. Established 1991.</obo:IAO_0000115>
        <oboInOwl:hasOBONamespace>GAZ</oboInOwl:hasOBONamespace>
        <oboInOwl:id>GAZ:00179221</oboInOwl:id>
        <rdfs:label>Aluvium Blhu</rdfs:label>
    </owl:NamedIndividual>
    


    <!-- http://purl.obolibrary.org/obo/GAZ_00179276 -->

    <owl:NamedIndividual rdf:about="http://purl.obolibrary.org/obo/GAZ_00179276">
        <obo:IAO_0000115>A reservoir upstream of Priboj.</obo:IAO_0000115>
        <oboInOwl:hasOBONamespace>GAZ</oboInOwl:hasOBONamespace>
        <oboInOwl:id>GAZ:00179276</oboInOwl:id>
        <rdfs:label>Lake Potpec</rdfs:label>
    </owl:NamedIndividual>
    


    <!-- http://purl.obolibrary.org/obo/GAZ_00179809 -->

    <owl:NamedIndividual rdf:about="http://purl.obolibrary.org/obo/GAZ_00179809">
        <obo:IAO_0000115>A hydroelectric dam. It is part of the Dalesice pumped-storage plant.</obo:IAO_0000115>
        <oboInOwl:hasOBONamespace>GAZ</oboInOwl:hasOBONamespace>
        <oboInOwl:id>GAZ:00179809</oboInOwl:id>
        <rdfs:label>Dalesice prehradni</rdfs:label>
    </owl:NamedIndividual>
    


    <!-- http://purl.obolibrary.org/obo/GAZ_00261043 -->

    <owl:NamedIndividual rdf:about="http://purl.obolibrary.org/obo/GAZ_00261043">
        <obo:IAO_0000115>A 43 km long river in Carinthia, Slovenia. It has its source on the Austrian side of the state border near Mount Olseva, becomes subterranean a kilometer from its source, and reappears on the surface in Koprivna near Crna na Koroskem, Slovenia. It is the central river of the Mezica Valley. It flows through Crna na Koroskem, Mezica, Prevalje, and Ravne na Koroskem, and into the Drava River at Dravograd.</obo:IAO_0000115>
        <oboInOwl:hasOBONamespace>GAZ</oboInOwl:hasOBONamespace>
        <oboInOwl:id>GAZ:00261043</oboInOwl:id>
        <rdfs:label>Meza</rdfs:label>
    </owl:NamedIndividual>
    


    <!-- http://purl.obolibrary.org/obo/GAZ_00261045 -->

    <owl:NamedIndividual rdf:about="http://purl.obolibrary.org/obo/GAZ_00261045">
        <obo:IAO_0000115>A river.</obo:IAO_0000115>
        <oboInOwl:hasOBONamespace>GAZ</oboInOwl:hasOBONamespace>
        <oboInOwl:id>GAZ:00261045</oboInOwl:id>
        <rdfs:label>Bednja</rdfs:label>
    </owl:NamedIndividual>
    


    <!-- http://purl.obolibrary.org/obo/GAZ_00261046 -->

    <owl:NamedIndividual rdf:about="http://purl.obolibrary.org/obo/GAZ_00261046">
        <obo:IAO_0000115>A river in Carinthia, Austria. A northern tributary of the river Drava, the 120 km long Gurk flows from under Nock Mountains, near the border of Austrian provinces of Styria and Carinthia. Its sources are two small lakes, the Gurksee and the Torersee, are located in two small cirques. It flows eastward through the Gurktal valley. Near Strassburg it turns southwards and flows into the Drava between Klagenfurt and Volkermarkt. Its tributaries include the Gortschitz, the Metnitz, and the Glan.</obo:IAO_0000115>
        <oboInOwl:hasOBONamespace>GAZ</oboInOwl:hasOBONamespace>
        <oboInOwl:id>GAZ:00261046</oboInOwl:id>
        <rdfs:label>Gurk</rdfs:label>
    </owl:NamedIndividual>
    


    <!-- http://purl.obolibrary.org/obo/GAZ_00261049 -->

    <owl:NamedIndividual rdf:about="http://purl.obolibrary.org/obo/GAZ_00261049">
        <obo:IAO_0000115>A river of Slovenia. The river is 40 km in length.</obo:IAO_0000115>
        <oboInOwl:hasOBONamespace>GAZ</oboInOwl:hasOBONamespace>
        <oboInOwl:id>GAZ:00261049</oboInOwl:id>
        <rdfs:label>Polskava</rdfs:label>
    </owl:NamedIndividual>
    


    <!-- http://purl.obolibrary.org/obo/GAZ_00360686 -->

    <owl:NamedIndividual rdf:about="http://purl.obolibrary.org/obo/GAZ_00360686">
        <obo:IAO_0000115>A river. A tributary of the Podriga River in Romania.</obo:IAO_0000115>
        <oboInOwl:hasOBONamespace>GAZ</oboInOwl:hasOBONamespace>
        <oboInOwl:id>GAZ:00360686</oboInOwl:id>
        <rdfs:label>Izvoarele</rdfs:label>
    </owl:NamedIndividual>
    


    <!-- http://purl.obolibrary.org/obo/GAZ_00360687 -->

    <owl:NamedIndividual rdf:about="http://purl.obolibrary.org/obo/GAZ_00360687">
        <obo:IAO_0000115>A river. A tributary of the Podriga River in Romania.</obo:IAO_0000115>
        <oboInOwl:hasOBONamespace>GAZ</oboInOwl:hasOBONamespace>
        <oboInOwl:id>GAZ:00360687</oboInOwl:id>
        <rdfs:label>Lismanita</rdfs:label>
    </owl:NamedIndividual>
    


    <!-- http://purl.obolibrary.org/obo/GAZ_00360688 -->

    <owl:NamedIndividual rdf:about="http://purl.obolibrary.org/obo/GAZ_00360688">
        <obo:IAO_0000115>A river. A tributary of the Podriga River in Romania.</obo:IAO_0000115>
        <oboInOwl:hasOBONamespace>GAZ</oboInOwl:hasOBONamespace>
        <oboInOwl:id>GAZ:00360688</oboInOwl:id>
        <rdfs:label>Valea Boului</rdfs:label>
    </owl:NamedIndividual>
    


    <!-- http://purl.obolibrary.org/obo/GAZ_00360729 -->

    <owl:NamedIndividual rdf:about="http://purl.obolibrary.org/obo/GAZ_00360729">
        <obo:IAO_0000115>A river.</obo:IAO_0000115>
        <oboInOwl:hasOBONamespace>GAZ</oboInOwl:hasOBONamespace>
        <oboInOwl:id>GAZ:00360729</oboInOwl:id>
        <rdfs:label>Roscani</rdfs:label>
    </owl:NamedIndividual>
    


    <!-- http://purl.obolibrary.org/obo/GAZ_00360730 -->

    <owl:NamedIndividual rdf:about="http://purl.obolibrary.org/obo/GAZ_00360730">
        <obo:IAO_0000115>A river.</obo:IAO_0000115>
        <oboInOwl:hasOBONamespace>GAZ</oboInOwl:hasOBONamespace>
        <oboInOwl:id>GAZ:00360730</oboInOwl:id>
        <rdfs:label>Radeni</rdfs:label>
    </owl:NamedIndividual>
    


    <!-- http://purl.obolibrary.org/obo/GAZ_00360731 -->

    <owl:NamedIndividual rdf:about="http://purl.obolibrary.org/obo/GAZ_00360731">
        <obo:IAO_0000115>A river.</obo:IAO_0000115>
        <oboInOwl:hasOBONamespace>GAZ</oboInOwl:hasOBONamespace>
        <oboInOwl:id>GAZ:00360731</oboInOwl:id>
        <rdfs:label>Optoceni</rdfs:label>
    </owl:NamedIndividual>
    


    <!-- http://purl.obolibrary.org/obo/GAZ_00360732 -->

    <owl:NamedIndividual rdf:about="http://purl.obolibrary.org/obo/GAZ_00360732">
        <obo:IAO_0000115>A river.</obo:IAO_0000115>
        <oboInOwl:hasOBONamespace>GAZ</oboInOwl:hasOBONamespace>
        <oboInOwl:id>GAZ:00360732</oboInOwl:id>
        <rdfs:label>Bahna</rdfs:label>
    </owl:NamedIndividual>
    


    <!-- http://purl.obolibrary.org/obo/GAZ_00360733 -->

    <owl:NamedIndividual rdf:about="http://purl.obolibrary.org/obo/GAZ_00360733">
        <obo:IAO_0000115>A river.</obo:IAO_0000115>
        <oboInOwl:hasOBONamespace>GAZ</oboInOwl:hasOBONamespace>
        <oboInOwl:id>GAZ:00360733</oboInOwl:id>
        <rdfs:label>Paraul Intors</rdfs:label>
    </owl:NamedIndividual>
    


    <!-- http://purl.obolibrary.org/obo/GAZ_00360737 -->

    <owl:NamedIndividual rdf:about="http://purl.obolibrary.org/obo/GAZ_00360737">
        <obo:IAO_0000115>A river.</obo:IAO_0000115>
        <oboInOwl:hasOBONamespace>GAZ</oboInOwl:hasOBONamespace>
        <oboInOwl:id>GAZ:00360737</oboInOwl:id>
        <rdfs:label>Ghilauca</rdfs:label>
    </owl:NamedIndividual>
    


    <!-- http://purl.obolibrary.org/obo/GAZ_00360738 -->

    <owl:NamedIndividual rdf:about="http://purl.obolibrary.org/obo/GAZ_00360738">
        <obo:IAO_0000115>A river.</obo:IAO_0000115>
        <oboInOwl:hasOBONamespace>GAZ</oboInOwl:hasOBONamespace>
        <oboInOwl:id>GAZ:00360738</oboInOwl:id>
        <rdfs:label>Vorniceasa</rdfs:label>
    </owl:NamedIndividual>
    


    <!-- http://purl.obolibrary.org/obo/GAZ_00360763 -->

    <owl:NamedIndividual rdf:about="http://purl.obolibrary.org/obo/GAZ_00360763">
        <obo:IAO_0000115>A river.</obo:IAO_0000115>
        <oboInOwl:hasOBONamespace>GAZ</oboInOwl:hasOBONamespace>
        <oboInOwl:id>GAZ:00360763</oboInOwl:id>
        <rdfs:label>Valea Reaa</rdfs:label>
    </owl:NamedIndividual>
    


    <!-- http://purl.obolibrary.org/obo/GAZ_00360764 -->

    <owl:NamedIndividual rdf:about="http://purl.obolibrary.org/obo/GAZ_00360764">
        <obo:IAO_0000115>A river.</obo:IAO_0000115>
        <oboInOwl:hasOBONamespace>GAZ</oboInOwl:hasOBONamespace>
        <oboInOwl:id>GAZ:00360764</oboInOwl:id>
        <rdfs:label>Paraul lui Vasile</rdfs:label>
    </owl:NamedIndividual>
    


    <!-- http://purl.obolibrary.org/obo/GAZ_00360765 -->

    <owl:NamedIndividual rdf:about="http://purl.obolibrary.org/obo/GAZ_00360765">
        <obo:IAO_0000115>A river.</obo:IAO_0000115>
        <oboInOwl:hasOBONamespace>GAZ</oboInOwl:hasOBONamespace>
        <oboInOwl:id>GAZ:00360765</oboInOwl:id>
        <rdfs:label>Recea</rdfs:label>
    </owl:NamedIndividual>
    


    <!-- http://purl.obolibrary.org/obo/GAZ_00360766 -->

    <owl:NamedIndividual rdf:about="http://purl.obolibrary.org/obo/GAZ_00360766">
        <obo:IAO_0000115>A river.</obo:IAO_0000115>
        <oboInOwl:hasOBONamespace>GAZ</oboInOwl:hasOBONamespace>
        <oboInOwl:id>GAZ:00360766</oboInOwl:id>
        <rdfs:label>Chirivoaia</rdfs:label>
    </owl:NamedIndividual>
    


    <!-- http://purl.obolibrary.org/obo/GAZ_00360767 -->

    <owl:NamedIndividual rdf:about="http://purl.obolibrary.org/obo/GAZ_00360767">
        <obo:IAO_0000115>A river.</obo:IAO_0000115>
        <oboInOwl:hasOBONamespace>GAZ</oboInOwl:hasOBONamespace>
        <oboInOwl:id>GAZ:00360767</oboInOwl:id>
        <rdfs:label>Raul Putred</rdfs:label>
    </owl:NamedIndividual>
    


    <!-- http://purl.obolibrary.org/obo/GAZ_00360768 -->

    <owl:NamedIndividual rdf:about="http://purl.obolibrary.org/obo/GAZ_00360768">
        <obo:IAO_0000115>A river.</obo:IAO_0000115>
        <oboInOwl:hasOBONamespace>GAZ</oboInOwl:hasOBONamespace>
        <oboInOwl:id>GAZ:00360768</oboInOwl:id>
        <rdfs:label>Oneaga</rdfs:label>
    </owl:NamedIndividual>
    


    <!-- http://purl.obolibrary.org/obo/GAZ_00360769 -->

    <owl:NamedIndividual rdf:about="http://purl.obolibrary.org/obo/GAZ_00360769">
        <obo:IAO_0000115>A river.</obo:IAO_0000115>
        <oboInOwl:hasOBONamespace>GAZ</oboInOwl:hasOBONamespace>
        <oboInOwl:id>GAZ:00360769</oboInOwl:id>
        <rdfs:label>Horoghiuca</rdfs:label>
    </owl:NamedIndividual>
    


    <!-- http://purl.obolibrary.org/obo/GAZ_00360770 -->

    <owl:NamedIndividual rdf:about="http://purl.obolibrary.org/obo/GAZ_00360770">
        <obo:IAO_0000115>A river.</obo:IAO_0000115>
        <oboInOwl:hasOBONamespace>GAZ</oboInOwl:hasOBONamespace>
        <oboInOwl:id>GAZ:00360770</oboInOwl:id>
        <rdfs:label>Varnita</rdfs:label>
    </owl:NamedIndividual>
    


    <!-- http://purl.obolibrary.org/obo/GAZ_00360771 -->

    <owl:NamedIndividual rdf:about="http://purl.obolibrary.org/obo/GAZ_00360771">
        <obo:IAO_0000115>A river.</obo:IAO_0000115>
        <oboInOwl:hasOBONamespace>GAZ</oboInOwl:hasOBONamespace>
        <oboInOwl:id>GAZ:00360771</oboInOwl:id>
        <rdfs:label>Scanteia</rdfs:label>
    </owl:NamedIndividual>
    


    <!-- http://purl.obolibrary.org/obo/GAZ_00360772 -->

    <owl:NamedIndividual rdf:about="http://purl.obolibrary.org/obo/GAZ_00360772">
        <obo:IAO_0000115>A river.</obo:IAO_0000115>
        <oboInOwl:hasOBONamespace>GAZ</oboInOwl:hasOBONamespace>
        <oboInOwl:id>GAZ:00360772</oboInOwl:id>
        <rdfs:label>La Moara de Vant</rdfs:label>
    </owl:NamedIndividual>
    


    <!-- http://purl.obolibrary.org/obo/GAZ_00360773 -->

    <owl:NamedIndividual rdf:about="http://purl.obolibrary.org/obo/GAZ_00360773">
        <obo:IAO_0000115>A river.</obo:IAO_0000115>
        <oboInOwl:hasOBONamespace>GAZ</oboInOwl:hasOBONamespace>
        <oboInOwl:id>GAZ:00360773</oboInOwl:id>
        <rdfs:label>Robu</rdfs:label>
    </owl:NamedIndividual>
    


    <!-- http://purl.obolibrary.org/obo/GAZ_00360826 -->

    <owl:NamedIndividual rdf:about="http://purl.obolibrary.org/obo/GAZ_00360826">
        <obo:IAO_0000115>A storage reservoir.</obo:IAO_0000115>
        <oboInOwl:hasOBONamespace>GAZ</oboInOwl:hasOBONamespace>
        <oboInOwl:id>GAZ:00360826</oboInOwl:id>
        <rdfs:label>Lake Plopi</rdfs:label>
    </owl:NamedIndividual>
    


    <!-- http://purl.obolibrary.org/obo/GAZ_00360827 -->

    <owl:NamedIndividual rdf:about="http://purl.obolibrary.org/obo/GAZ_00360827">
        <obo:IAO_0000115>A dam.</obo:IAO_0000115>
        <oboInOwl:hasOBONamespace>GAZ</oboInOwl:hasOBONamespace>
        <oboInOwl:id>GAZ:00360827</oboInOwl:id>
        <rdfs:label>Vanatori Dam</rdfs:label>
    </owl:NamedIndividual>
    


    <!-- http://purl.obolibrary.org/obo/GAZ_00360828 -->

    <owl:NamedIndividual rdf:about="http://purl.obolibrary.org/obo/GAZ_00360828">
        <obo:IAO_0000115>A dam.</obo:IAO_0000115>
        <oboInOwl:hasOBONamespace>GAZ</oboInOwl:hasOBONamespace>
        <oboInOwl:id>GAZ:00360828</oboInOwl:id>
        <rdfs:label>Carlig Dam</rdfs:label>
    </owl:NamedIndividual>
    


    <!-- http://purl.obolibrary.org/obo/GAZ_00360834 -->

    <owl:NamedIndividual rdf:about="http://purl.obolibrary.org/obo/GAZ_00360834">
        <obo:IAO_0000115>A lake.</obo:IAO_0000115>
        <oboInOwl:hasOBONamespace>GAZ</oboInOwl:hasOBONamespace>
        <oboInOwl:id>GAZ:00360834</oboInOwl:id>
        <rdfs:label>Lake Ciric I</rdfs:label>
    </owl:NamedIndividual>
    


    <!-- http://purl.obolibrary.org/obo/GAZ_00360835 -->

    <owl:NamedIndividual rdf:about="http://purl.obolibrary.org/obo/GAZ_00360835">
        <obo:IAO_0000115>A lake.</obo:IAO_0000115>
        <oboInOwl:hasOBONamespace>GAZ</oboInOwl:hasOBONamespace>
        <oboInOwl:id>GAZ:00360835</oboInOwl:id>
        <rdfs:label>Lake Ciric II</rdfs:label>
    </owl:NamedIndividual>
    


    <!-- http://purl.obolibrary.org/obo/GAZ_00360836 -->

    <owl:NamedIndividual rdf:about="http://purl.obolibrary.org/obo/GAZ_00360836">
        <obo:IAO_0000115>A lake.</obo:IAO_0000115>
        <oboInOwl:hasOBONamespace>GAZ</oboInOwl:hasOBONamespace>
        <oboInOwl:id>GAZ:00360836</oboInOwl:id>
        <rdfs:label>Lake Ciric III</rdfs:label>
    </owl:NamedIndividual>
    


    <!-- http://purl.obolibrary.org/obo/GAZ_00360837 -->

    <owl:NamedIndividual rdf:about="http://purl.obolibrary.org/obo/GAZ_00360837">
        <obo:IAO_0000115>A river.</obo:IAO_0000115>
        <oboInOwl:hasOBONamespace>GAZ</oboInOwl:hasOBONamespace>
        <oboInOwl:id>GAZ:00360837</oboInOwl:id>
        <rdfs:label>Valea Lunga</rdfs:label>
    </owl:NamedIndividual>
    


    <!-- http://purl.obolibrary.org/obo/GAZ_00360855 -->

    <owl:NamedIndividual rdf:about="http://purl.obolibrary.org/obo/GAZ_00360855">
        <obo:IAO_0000115>A river.</obo:IAO_0000115>
        <oboInOwl:hasOBONamespace>GAZ</oboInOwl:hasOBONamespace>
        <oboInOwl:id>GAZ:00360855</oboInOwl:id>
        <rdfs:label>Todiresti</rdfs:label>
    </owl:NamedIndividual>
    


    <!-- http://purl.obolibrary.org/obo/GAZ_00360856 -->

    <owl:NamedIndividual rdf:about="http://purl.obolibrary.org/obo/GAZ_00360856">
        <obo:IAO_0000115>A river.</obo:IAO_0000115>
        <oboInOwl:hasOBONamespace>GAZ</oboInOwl:hasOBONamespace>
        <oboInOwl:id>GAZ:00360856</oboInOwl:id>
        <rdfs:label>Recea</rdfs:label>
    </owl:NamedIndividual>
    


    <!-- http://purl.obolibrary.org/obo/GAZ_00360857 -->

    <owl:NamedIndividual rdf:about="http://purl.obolibrary.org/obo/GAZ_00360857">
        <obo:IAO_0000115>A storage reservoir.</obo:IAO_0000115>
        <oboInOwl:hasOBONamespace>GAZ</oboInOwl:hasOBONamespace>
        <oboInOwl:id>GAZ:00360857</oboInOwl:id>
        <rdfs:label>Sarca Reservoir</rdfs:label>
    </owl:NamedIndividual>
    


    <!-- http://purl.obolibrary.org/obo/GAZ_00360858 -->

    <owl:NamedIndividual rdf:about="http://purl.obolibrary.org/obo/GAZ_00360858">
        <obo:IAO_0000115>A river.</obo:IAO_0000115>
        <oboInOwl:hasOBONamespace>GAZ</oboInOwl:hasOBONamespace>
        <oboInOwl:id>GAZ:00360858</oboInOwl:id>
        <rdfs:label>Strunga</rdfs:label>
    </owl:NamedIndividual>
    


    <!-- http://purl.obolibrary.org/obo/GAZ_00360870 -->

    <owl:NamedIndividual rdf:about="http://purl.obolibrary.org/obo/GAZ_00360870">
        <obo:IAO_0000115>A lake.</obo:IAO_0000115>
        <oboInOwl:hasOBONamespace>GAZ</oboInOwl:hasOBONamespace>
        <oboInOwl:id>GAZ:00360870</oboInOwl:id>
        <rdfs:label>Lake Dumesti I</rdfs:label>
    </owl:NamedIndividual>
    


    <!-- http://purl.obolibrary.org/obo/GAZ_00360871 -->

    <owl:NamedIndividual rdf:about="http://purl.obolibrary.org/obo/GAZ_00360871">
        <obo:IAO_0000115>A lake.</obo:IAO_0000115>
        <oboInOwl:hasOBONamespace>GAZ</oboInOwl:hasOBONamespace>
        <oboInOwl:id>GAZ:00360871</oboInOwl:id>
        <rdfs:label>Lake Pausesti</rdfs:label>
    </owl:NamedIndividual>
    


    <!-- http://purl.obolibrary.org/obo/GAZ_00360872 -->

    <owl:NamedIndividual rdf:about="http://purl.obolibrary.org/obo/GAZ_00360872">
        <obo:IAO_0000115>A river.</obo:IAO_0000115>
        <oboInOwl:hasOBONamespace>GAZ</oboInOwl:hasOBONamespace>
        <oboInOwl:id>GAZ:00360872</oboInOwl:id>
        <rdfs:label>Boghea</rdfs:label>
    </owl:NamedIndividual>
    


    <!-- http://purl.obolibrary.org/obo/GAZ_00360873 -->

    <owl:NamedIndividual rdf:about="http://purl.obolibrary.org/obo/GAZ_00360873">
        <obo:IAO_0000115>A river.</obo:IAO_0000115>
        <oboInOwl:hasOBONamespace>GAZ</oboInOwl:hasOBONamespace>
        <oboInOwl:id>GAZ:00360873</oboInOwl:id>
        <rdfs:label>Cornesti</rdfs:label>
    </owl:NamedIndividual>
    


    <!-- http://purl.obolibrary.org/obo/GAZ_00360874 -->

    <owl:NamedIndividual rdf:about="http://purl.obolibrary.org/obo/GAZ_00360874">
        <obo:IAO_0000115>A river.</obo:IAO_0000115>
        <oboInOwl:hasOBONamespace>GAZ</oboInOwl:hasOBONamespace>
        <oboInOwl:id>GAZ:00360874</oboInOwl:id>
        <rdfs:label>Valea Adanca</rdfs:label>
    </owl:NamedIndividual>
    


    <!-- http://purl.obolibrary.org/obo/GAZ_00360879 -->

    <owl:NamedIndividual rdf:about="http://purl.obolibrary.org/obo/GAZ_00360879">
        <obo:IAO_0000115>A dam.</obo:IAO_0000115>
        <oboInOwl:hasOBONamespace>GAZ</oboInOwl:hasOBONamespace>
        <oboInOwl:id>GAZ:00360879</oboInOwl:id>
        <rdfs:label>Cornet Dama</rdfs:label>
    </owl:NamedIndividual>
    


    <!-- http://purl.obolibrary.org/obo/GAZ_00360880 -->

    <owl:NamedIndividual rdf:about="http://purl.obolibrary.org/obo/GAZ_00360880">
        <obo:IAO_0000115>A dam.</obo:IAO_0000115>
        <oboInOwl:hasOBONamespace>GAZ</oboInOwl:hasOBONamespace>
        <oboInOwl:id>GAZ:00360880</oboInOwl:id>
        <rdfs:label>Ezareni Dam</rdfs:label>
    </owl:NamedIndividual>
    


    <!-- http://purl.obolibrary.org/obo/GAZ_00360883 -->

    <owl:NamedIndividual rdf:about="http://purl.obolibrary.org/obo/GAZ_00360883">
        <obo:IAO_0000115>A lake.</obo:IAO_0000115>
        <oboInOwl:hasOBONamespace>GAZ</oboInOwl:hasOBONamespace>
        <oboInOwl:id>GAZ:00360883</oboInOwl:id>
        <rdfs:label>Lacul Beleu</rdfs:label>
    </owl:NamedIndividual>
    


    <!-- http://purl.obolibrary.org/obo/GAZ_00360891 -->

    <owl:NamedIndividual rdf:about="http://purl.obolibrary.org/obo/GAZ_00360891">
        <obo:IAO_0000115>A river.</obo:IAO_0000115>
        <oboInOwl:hasOBONamespace>GAZ</oboInOwl:hasOBONamespace>
        <oboInOwl:id>GAZ:00360891</oboInOwl:id>
        <rdfs:label>Limpeioara</rdfs:label>
    </owl:NamedIndividual>
    


    <!-- http://purl.obolibrary.org/obo/GAZ_00360892 -->

    <owl:NamedIndividual rdf:about="http://purl.obolibrary.org/obo/GAZ_00360892">
        <obo:IAO_0000115>A river.</obo:IAO_0000115>
        <oboInOwl:hasOBONamespace>GAZ</oboInOwl:hasOBONamespace>
        <oboInOwl:id>GAZ:00360892</oboInOwl:id>
        <rdfs:label>Tincuta</rdfs:label>
    </owl:NamedIndividual>
    


    <!-- http://purl.obolibrary.org/obo/GAZ_00360941 -->

    <owl:NamedIndividual rdf:about="http://purl.obolibrary.org/obo/GAZ_00360941">
        <obo:RO_0001025 rdf:resource="http://purl.obolibrary.org/obo/GAZ_00360942"/>
        <obo:IAO_0000115>A man-made lake.</obo:IAO_0000115>
        <oboInOwl:hasOBONamespace>GAZ</oboInOwl:hasOBONamespace>
        <oboInOwl:id>GAZ:00360941</oboInOwl:id>
        <rdfs:label>Lacul Sireti-Ghidighici</rdfs:label>
    </owl:NamedIndividual>
    


    <!-- http://purl.obolibrary.org/obo/GAZ_00360942 -->

    <owl:NamedIndividual rdf:about="http://purl.obolibrary.org/obo/GAZ_00360942">
        <obo:IAO_0000115>A river.</obo:IAO_0000115>
        <oboInOwl:hasOBONamespace>GAZ</oboInOwl:hasOBONamespace>
        <oboInOwl:id>GAZ:00360942</oboInOwl:id>
        <rdfs:label>Raul Bic</rdfs:label>
    </owl:NamedIndividual>
    


    <!-- http://purl.obolibrary.org/obo/GAZ_00360951 -->

    <owl:NamedIndividual rdf:about="http://purl.obolibrary.org/obo/GAZ_00360951">
        <obo:IAO_0000115>A lake.</obo:IAO_0000115>
        <oboInOwl:hasOBONamespace>GAZ</oboInOwl:hasOBONamespace>
        <oboInOwl:id>GAZ:00360951</oboInOwl:id>
        <rdfs:label>Lacul Manta</rdfs:label>
    </owl:NamedIndividual>
    


    <!-- http://purl.obolibrary.org/obo/GAZ_00360989 -->

    <owl:NamedIndividual rdf:about="http://purl.obolibrary.org/obo/GAZ_00360989">
        <obo:RO_0001025 rdf:resource="http://purl.obolibrary.org/obo/GAZ_00042218"/>
        <obo:IAO_0000115>A lake.</obo:IAO_0000115>
        <oboInOwl:hasOBONamespace>GAZ</oboInOwl:hasOBONamespace>
        <oboInOwl:id>GAZ:00360989</oboInOwl:id>
        <rdfs:label>Lacul Kugurluy</rdfs:label>
    </owl:NamedIndividual>
    


    <!-- http://purl.obolibrary.org/obo/GAZ_00360990 -->

    <owl:NamedIndividual rdf:about="http://purl.obolibrary.org/obo/GAZ_00360990">
        <obo:RO_0001025 rdf:resource="http://purl.obolibrary.org/obo/GAZ_00042218"/>
        <obo:IAO_0000115>A distributary of the river Danube, that contributes in forming the Danube Delta.</obo:IAO_0000115>
        <oboInOwl:hasOBONamespace>GAZ</oboInOwl:hasOBONamespace>
        <oboInOwl:id>GAZ:00360990</oboInOwl:id>
        <rdfs:label>Chilia branch</rdfs:label>
    </owl:NamedIndividual>
    


    <!-- http://purl.obolibrary.org/obo/GAZ_00360991 -->

    <owl:NamedIndividual rdf:about="http://purl.obolibrary.org/obo/GAZ_00360991">
        <obo:RO_0001025 rdf:resource="http://purl.obolibrary.org/obo/GAZ_00042218"/>
        <obo:IAO_0000115>A distributary of the river Danube.</obo:IAO_0000115>
        <oboInOwl:hasOBONamespace>GAZ</oboInOwl:hasOBONamespace>
        <oboInOwl:id>GAZ:00360991</oboInOwl:id>
        <rdfs:label>Sulina branch</rdfs:label>
    </owl:NamedIndividual>
    


    <!-- http://purl.obolibrary.org/obo/GAZ_00362903 -->

    <owl:NamedIndividual rdf:about="http://purl.obolibrary.org/obo/GAZ_00362903">
        <obo:RO_0001025 rdf:resource="http://purl.obolibrary.org/obo/GAZ_00143922"/>
        <obo:IAO_0000115>A river.</obo:IAO_0000115>
        <oboInOwl:hasOBONamespace>GAZ</oboInOwl:hasOBONamespace>
        <oboInOwl:id>GAZ:00362903</oboInOwl:id>
        <rdfs:label>Piva</rdfs:label>
    </owl:NamedIndividual>
    


    <!-- http://purl.obolibrary.org/obo/GAZ_00362927 -->

    <owl:NamedIndividual rdf:about="http://purl.obolibrary.org/obo/GAZ_00362927">
        <obo:RO_0001025 rdf:resource="http://purl.obolibrary.org/obo/GAZ_00362903"/>
        <obo:IAO_0000115>A man-made lake. Impounded by Mratinje Dam. Constructed 1975.</obo:IAO_0000115>
        <oboInOwl:hasOBONamespace>GAZ</oboInOwl:hasOBONamespace>
        <oboInOwl:id>GAZ:00362927</oboInOwl:id>
        <rdfs:label>Lake Piva</rdfs:label>
    </owl:NamedIndividual>
    


    <!-- http://purl.obolibrary.org/obo/GAZ_00362928 -->

    <owl:NamedIndividual rdf:about="http://purl.obolibrary.org/obo/GAZ_00362928">
        <obo:RO_0001025 rdf:resource="http://purl.obolibrary.org/obo/GAZ_00362903"/>
        <obo:IAO_0000115>A concrete arch-gravity dam in the canyon of the Piva River in Montenegro. Completed 1975.</obo:IAO_0000115>
        <oboInOwl:hasOBONamespace>GAZ</oboInOwl:hasOBONamespace>
        <oboInOwl:id>GAZ:00362928</oboInOwl:id>
        <rdfs:label>Mratinje Dam</rdfs:label>
    </owl:NamedIndividual>
    


    <!-- http://purl.obolibrary.org/obo/GAZ_00362971 -->

    <owl:NamedIndividual rdf:about="http://purl.obolibrary.org/obo/GAZ_00362971">
        <obo:IAO_0000115>A river.</obo:IAO_0000115>
        <oboInOwl:hasOBONamespace>GAZ</oboInOwl:hasOBONamespace>
        <oboInOwl:id>GAZ:00362971</oboInOwl:id>
        <rdfs:label>Savnik</rdfs:label>
    </owl:NamedIndividual>
    


    <!-- http://purl.obolibrary.org/obo/GAZ_00362989 -->

    <owl:NamedIndividual rdf:about="http://purl.obolibrary.org/obo/GAZ_00362989">
        <obo:IAO_0000115>An artificial lake on the Sokobanjska Moravica.</obo:IAO_0000115>
        <oboInOwl:hasOBONamespace>GAZ</oboInOwl:hasOBONamespace>
        <oboInOwl:id>GAZ:00362989</oboInOwl:id>
        <rdfs:label>Lake Bovan</rdfs:label>
    </owl:NamedIndividual>
    


    <!-- http://purl.obolibrary.org/obo/GAZ_00363029 -->

    <owl:NamedIndividual rdf:about="http://purl.obolibrary.org/obo/GAZ_00363029">
        <obo:IAO_0000115>A river.</obo:IAO_0000115>
        <oboInOwl:hasOBONamespace>GAZ</oboInOwl:hasOBONamespace>
        <oboInOwl:id>GAZ:00363029</oboInOwl:id>
        <rdfs:label>Beljeva</rdfs:label>
    </owl:NamedIndividual>
    


    <!-- http://purl.obolibrary.org/obo/GAZ_00363033 -->

    <owl:NamedIndividual rdf:about="http://purl.obolibrary.org/obo/GAZ_00363033">
        <oboInOwl:hasOBONamespace>GAZ</oboInOwl:hasOBONamespace>
        <oboInOwl:id>GAZ:00363033</oboInOwl:id>
        <rdfs:label>Dulensko jezero</rdfs:label>
    </owl:NamedIndividual>
    


    <!-- http://purl.obolibrary.org/obo/GAZ_00363034 -->

    <owl:NamedIndividual rdf:about="http://purl.obolibrary.org/obo/GAZ_00363034">
        <obo:IAO_0000115>A man-made lake.</obo:IAO_0000115>
        <oboInOwl:hasOBONamespace>GAZ</oboInOwl:hasOBONamespace>
        <oboInOwl:id>GAZ:00363034</oboInOwl:id>
        <rdfs:label>Grosnica</rdfs:label>
    </owl:NamedIndividual>
    


    <!-- http://purl.obolibrary.org/obo/GAZ_00368181 -->

    <owl:NamedIndividual rdf:about="http://purl.obolibrary.org/obo/GAZ_00368181">
        <obo:IAO_0000115>A river.</obo:IAO_0000115>
        <oboInOwl:hasOBONamespace>GAZ</oboInOwl:hasOBONamespace>
        <oboInOwl:id>GAZ:00368181</oboInOwl:id>
        <rdfs:label>Bega</rdfs:label>
    </owl:NamedIndividual>
    


    <!-- http://purl.obolibrary.org/obo/GAZ_00368313 -->

    <owl:NamedIndividual rdf:about="http://purl.obolibrary.org/obo/GAZ_00368313">
        <oboInOwl:hasOBONamespace>GAZ</oboInOwl:hasOBONamespace>
        <oboInOwl:id>GAZ:00368313</oboInOwl:id>
        <rdfs:label>Valiug</rdfs:label>
    </owl:NamedIndividual>
    


    <!-- http://purl.obolibrary.org/obo/GAZ_00368336 -->

    <owl:NamedIndividual rdf:about="http://purl.obolibrary.org/obo/GAZ_00368336">
        <obo:IAO_0000115>A man-made lake.</obo:IAO_0000115>
        <oboInOwl:hasOBONamespace>GAZ</oboInOwl:hasOBONamespace>
        <oboInOwl:id>GAZ:00368336</oboInOwl:id>
        <rdfs:label>Lacul Breazova</rdfs:label>
    </owl:NamedIndividual>
    


    <!-- http://purl.obolibrary.org/obo/GAZ_00368352 -->

    <owl:NamedIndividual rdf:about="http://purl.obolibrary.org/obo/GAZ_00368352">
        <obo:IAO_0000115>A system of slow canals in the marshes of the lower Pancevacki Rit. It originates south of Borca and flows to the east, curving north of Kotez, bog of Veliko Blato, eastern Krnjacca and bogs of Sebes and Reva, before it empties into the Danube as its left tributary.</obo:IAO_0000115>
        <oboInOwl:hasOBONamespace>GAZ</oboInOwl:hasOBONamespace>
        <oboInOwl:id>GAZ:00368352</oboInOwl:id>
        <rdfs:label>Sebes [River]</rdfs:label>
    </owl:NamedIndividual>
    


    <!-- http://purl.obolibrary.org/obo/GAZ_00368358 -->

    <owl:NamedIndividual rdf:about="http://purl.obolibrary.org/obo/GAZ_00368358">
        <obo:IAO_0000115>A river.</obo:IAO_0000115>
        <oboInOwl:hasOBONamespace>GAZ</oboInOwl:hasOBONamespace>
        <oboInOwl:id>GAZ:00368358</oboInOwl:id>
        <rdfs:label>Ljubljanica</rdfs:label>
    </owl:NamedIndividual>
    


    <!-- http://purl.obolibrary.org/obo/GAZ_00368395 -->

    <owl:NamedIndividual rdf:about="http://purl.obolibrary.org/obo/GAZ_00368395">
        <obo:IAO_0000115>A mna-made lake.</obo:IAO_0000115>
        <oboInOwl:hasOBONamespace>GAZ</oboInOwl:hasOBONamespace>
        <oboInOwl:id>GAZ:00368395</oboInOwl:id>
        <rdfs:label>Pariguz</rdfs:label>
    </owl:NamedIndividual>
    


    <!-- http://purl.obolibrary.org/obo/GAZ_00368497 -->

    <owl:NamedIndividual rdf:about="http://purl.obolibrary.org/obo/GAZ_00368497">
        <obo:IAO_0000115>A river. It first flows through Lake Buhui. Thereafter it flows through the Buhui Cave and, after emerging from the cave, flows through a reach of narrow gorges before joining the Caras River.</obo:IAO_0000115>
        <oboInOwl:hasOBONamespace>GAZ</oboInOwl:hasOBONamespace>
        <oboInOwl:id>GAZ:00368497</oboInOwl:id>
        <rdfs:label>Buhui</rdfs:label>
    </owl:NamedIndividual>
    


    <!-- http://purl.obolibrary.org/obo/GAZ_00368498 -->

    <owl:NamedIndividual rdf:about="http://purl.obolibrary.org/obo/GAZ_00368498">
        <obo:IAO_0000115>A river.</obo:IAO_0000115>
        <oboInOwl:hasOBONamespace>GAZ</oboInOwl:hasOBONamespace>
        <oboInOwl:id>GAZ:00368498</oboInOwl:id>
        <rdfs:label>Raicovacea</rdfs:label>
    </owl:NamedIndividual>
    


    <!-- http://purl.obolibrary.org/obo/GAZ_00368499 -->

    <owl:NamedIndividual rdf:about="http://purl.obolibrary.org/obo/GAZ_00368499">
        <obo:IAO_0000115>A river.</obo:IAO_0000115>
        <oboInOwl:hasOBONamespace>GAZ</oboInOwl:hasOBONamespace>
        <oboInOwl:id>GAZ:00368499</oboInOwl:id>
        <rdfs:label>Sereniac</rdfs:label>
    </owl:NamedIndividual>
    


    <!-- http://purl.obolibrary.org/obo/GAZ_00368500 -->

    <owl:NamedIndividual rdf:about="http://purl.obolibrary.org/obo/GAZ_00368500">
        <obo:IAO_0000115>A river.</obo:IAO_0000115>
        <oboInOwl:hasOBONamespace>GAZ</oboInOwl:hasOBONamespace>
        <oboInOwl:id>GAZ:00368500</oboInOwl:id>
        <rdfs:label>Garliste</rdfs:label>
    </owl:NamedIndividual>
    


    <!-- http://purl.obolibrary.org/obo/GAZ_00368501 -->

    <owl:NamedIndividual rdf:about="http://purl.obolibrary.org/obo/GAZ_00368501">
        <obo:IAO_0000115>A river.</obo:IAO_0000115>
        <oboInOwl:hasOBONamespace>GAZ</oboInOwl:hasOBONamespace>
        <oboInOwl:id>GAZ:00368501</oboInOwl:id>
        <rdfs:label>Goruia</rdfs:label>
    </owl:NamedIndividual>
    


    <!-- http://purl.obolibrary.org/obo/GAZ_00368502 -->

    <owl:NamedIndividual rdf:about="http://purl.obolibrary.org/obo/GAZ_00368502">
        <obo:IAO_0000115>A river.</obo:IAO_0000115>
        <oboInOwl:hasOBONamespace>GAZ</oboInOwl:hasOBONamespace>
        <oboInOwl:id>GAZ:00368502</oboInOwl:id>
        <rdfs:label>Jitin</rdfs:label>
    </owl:NamedIndividual>
    


    <!-- http://purl.obolibrary.org/obo/GAZ_00368503 -->

    <owl:NamedIndividual rdf:about="http://purl.obolibrary.org/obo/GAZ_00368503">
        <obo:IAO_0000115>A river.</obo:IAO_0000115>
        <oboInOwl:hasOBONamespace>GAZ</oboInOwl:hasOBONamespace>
        <oboInOwl:id>GAZ:00368503</oboInOwl:id>
        <rdfs:label>Lisava</rdfs:label>
    </owl:NamedIndividual>
    


    <!-- http://purl.obolibrary.org/obo/GAZ_00368504 -->

    <owl:NamedIndividual rdf:about="http://purl.obolibrary.org/obo/GAZ_00368504">
        <obo:IAO_0000115>A river.</obo:IAO_0000115>
        <oboInOwl:hasOBONamespace>GAZ</oboInOwl:hasOBONamespace>
        <oboInOwl:id>GAZ:00368504</oboInOwl:id>
        <rdfs:label>Bucovat</rdfs:label>
    </owl:NamedIndividual>
    


    <!-- http://purl.obolibrary.org/obo/GAZ_00368505 -->

    <owl:NamedIndividual rdf:about="http://purl.obolibrary.org/obo/GAZ_00368505">
        <obo:IAO_0000115>A river.</obo:IAO_0000115>
        <oboInOwl:hasOBONamespace>GAZ</oboInOwl:hasOBONamespace>
        <oboInOwl:id>GAZ:00368505</oboInOwl:id>
        <rdfs:label>Ciclova</rdfs:label>
    </owl:NamedIndividual>
    


    <!-- http://purl.obolibrary.org/obo/GAZ_00368506 -->

    <owl:NamedIndividual rdf:about="http://purl.obolibrary.org/obo/GAZ_00368506">
        <obo:IAO_0000115>A river.</obo:IAO_0000115>
        <oboInOwl:hasOBONamespace>GAZ</oboInOwl:hasOBONamespace>
        <oboInOwl:id>GAZ:00368506</oboInOwl:id>
        <rdfs:label>Vicinic</rdfs:label>
    </owl:NamedIndividual>
    


    <!-- http://purl.obolibrary.org/obo/GAZ_00368507 -->

    <owl:NamedIndividual rdf:about="http://purl.obolibrary.org/obo/GAZ_00368507">
        <obo:IAO_0000115>A river.</obo:IAO_0000115>
        <oboInOwl:hasOBONamespace>GAZ</oboInOwl:hasOBONamespace>
        <oboInOwl:id>GAZ:00368507</oboInOwl:id>
        <rdfs:label>Ilidia</rdfs:label>
    </owl:NamedIndividual>
    


    <!-- http://purl.obolibrary.org/obo/GAZ_00368508 -->

    <owl:NamedIndividual rdf:about="http://purl.obolibrary.org/obo/GAZ_00368508">
        <obo:IAO_0000115>A river.</obo:IAO_0000115>
        <oboInOwl:hasOBONamespace>GAZ</oboInOwl:hasOBONamespace>
        <oboInOwl:id>GAZ:00368508</oboInOwl:id>
        <rdfs:label>Izvoru Mare</rdfs:label>
    </owl:NamedIndividual>
    


    <!-- http://purl.obolibrary.org/obo/GAZ_00368509 -->

    <owl:NamedIndividual rdf:about="http://purl.obolibrary.org/obo/GAZ_00368509">
        <obo:IAO_0000115>A river.</obo:IAO_0000115>
        <oboInOwl:hasOBONamespace>GAZ</oboInOwl:hasOBONamespace>
        <oboInOwl:id>GAZ:00368509</oboInOwl:id>
        <rdfs:label>Jervanu Mare</rdfs:label>
    </owl:NamedIndividual>
    


    <!-- http://purl.obolibrary.org/obo/GAZ_00368510 -->

    <owl:NamedIndividual rdf:about="http://purl.obolibrary.org/obo/GAZ_00368510">
        <obo:IAO_0000115>A river.</obo:IAO_0000115>
        <oboInOwl:hasOBONamespace>GAZ</oboInOwl:hasOBONamespace>
        <oboInOwl:id>GAZ:00368510</oboInOwl:id>
        <rdfs:label>Comarnic</rdfs:label>
    </owl:NamedIndividual>
    


    <!-- http://purl.obolibrary.org/obo/GAZ_00368511 -->

    <owl:NamedIndividual rdf:about="http://purl.obolibrary.org/obo/GAZ_00368511">
        <obo:IAO_0000115>A river.</obo:IAO_0000115>
        <oboInOwl:hasOBONamespace>GAZ</oboInOwl:hasOBONamespace>
        <oboInOwl:id>GAZ:00368511</oboInOwl:id>
        <rdfs:label>Gelug</rdfs:label>
    </owl:NamedIndividual>
    


    <!-- http://purl.obolibrary.org/obo/GAZ_00368512 -->

    <owl:NamedIndividual rdf:about="http://purl.obolibrary.org/obo/GAZ_00368512">
        <obo:IAO_0000115>A river.</obo:IAO_0000115>
        <oboInOwl:hasOBONamespace>GAZ</oboInOwl:hasOBONamespace>
        <oboInOwl:id>GAZ:00368512</oboInOwl:id>
        <rdfs:label>Dognecea</rdfs:label>
    </owl:NamedIndividual>
    


    <!-- http://purl.obolibrary.org/obo/GAZ_00368513 -->

    <owl:NamedIndividual rdf:about="http://purl.obolibrary.org/obo/GAZ_00368513">
        <obo:IAO_0000115>A river.</obo:IAO_0000115>
        <oboInOwl:hasOBONamespace>GAZ</oboInOwl:hasOBONamespace>
        <oboInOwl:id>GAZ:00368513</oboInOwl:id>
        <rdfs:label>Barches</rdfs:label>
    </owl:NamedIndividual>
    


    <!-- http://purl.obolibrary.org/obo/GAZ_00368514 -->

    <owl:NamedIndividual rdf:about="http://purl.obolibrary.org/obo/GAZ_00368514">
        <obo:IAO_0000115>A river.</obo:IAO_0000115>
        <oboInOwl:hasOBONamespace>GAZ</oboInOwl:hasOBONamespace>
        <oboInOwl:id>GAZ:00368514</oboInOwl:id>
        <rdfs:label>Cernovat</rdfs:label>
    </owl:NamedIndividual>
    


    <!-- http://purl.obolibrary.org/obo/GAZ_00368516 -->

    <owl:NamedIndividual rdf:about="http://purl.obolibrary.org/obo/GAZ_00368516">
        <obo:IAO_0000115>A river.</obo:IAO_0000115>
        <oboInOwl:hasOBONamespace>GAZ</oboInOwl:hasOBONamespace>
        <oboInOwl:id>GAZ:00368516</oboInOwl:id>
        <rdfs:label>Versteag</rdfs:label>
    </owl:NamedIndividual>
    


    <!-- http://purl.obolibrary.org/obo/GAZ_00368517 -->

    <owl:NamedIndividual rdf:about="http://purl.obolibrary.org/obo/GAZ_00368517">
        <obo:IAO_0000115>A river.</obo:IAO_0000115>
        <oboInOwl:hasOBONamespace>GAZ</oboInOwl:hasOBONamespace>
        <oboInOwl:id>GAZ:00368517</oboInOwl:id>
        <rdfs:label>Glavan</rdfs:label>
    </owl:NamedIndividual>
    


    <!-- http://purl.obolibrary.org/obo/GAZ_00368518 -->

    <owl:NamedIndividual rdf:about="http://purl.obolibrary.org/obo/GAZ_00368518">
        <obo:IAO_0000115>A river.</obo:IAO_0000115>
        <oboInOwl:hasOBONamespace>GAZ</oboInOwl:hasOBONamespace>
        <oboInOwl:id>GAZ:00368518</oboInOwl:id>
        <rdfs:label>Certet</rdfs:label>
    </owl:NamedIndividual>
    


    <!-- http://purl.obolibrary.org/obo/GAZ_00368519 -->

    <owl:NamedIndividual rdf:about="http://purl.obolibrary.org/obo/GAZ_00368519">
        <obo:IAO_0000115>A river.</obo:IAO_0000115>
        <oboInOwl:hasOBONamespace>GAZ</oboInOwl:hasOBONamespace>
        <oboInOwl:id>GAZ:00368519</oboInOwl:id>
        <rdfs:label>Terezia</rdfs:label>
    </owl:NamedIndividual>
    


    <!-- http://purl.obolibrary.org/obo/GAZ_00368520 -->

    <owl:NamedIndividual rdf:about="http://purl.obolibrary.org/obo/GAZ_00368520">
        <obo:IAO_0000115>A river.</obo:IAO_0000115>
        <oboInOwl:hasOBONamespace>GAZ</oboInOwl:hasOBONamespace>
        <oboInOwl:id>GAZ:00368520</oboInOwl:id>
        <rdfs:label>Valea Mare</rdfs:label>
    </owl:NamedIndividual>
    


    <!-- http://purl.obolibrary.org/obo/GAZ_00368521 -->

    <owl:NamedIndividual rdf:about="http://purl.obolibrary.org/obo/GAZ_00368521">
        <obo:IAO_0000115>A river.</obo:IAO_0000115>
        <oboInOwl:hasOBONamespace>GAZ</oboInOwl:hasOBONamespace>
        <oboInOwl:id>GAZ:00368521</oboInOwl:id>
        <rdfs:label>Celnicu Mare</rdfs:label>
    </owl:NamedIndividual>
    


    <!-- http://purl.obolibrary.org/obo/GAZ_00368522 -->

    <owl:NamedIndividual rdf:about="http://purl.obolibrary.org/obo/GAZ_00368522">
        <obo:IAO_0000115>A river.</obo:IAO_0000115>
        <oboInOwl:hasOBONamespace>GAZ</oboInOwl:hasOBONamespace>
        <oboInOwl:id>GAZ:00368522</oboInOwl:id>
        <rdfs:label>Celnicu Mic</rdfs:label>
    </owl:NamedIndividual>
    


    <!-- http://purl.obolibrary.org/obo/GAZ_00368523 -->

    <owl:NamedIndividual rdf:about="http://purl.obolibrary.org/obo/GAZ_00368523">
        <obo:IAO_0000115>A river.</obo:IAO_0000115>
        <oboInOwl:hasOBONamespace>GAZ</oboInOwl:hasOBONamespace>
        <oboInOwl:id>GAZ:00368523</oboInOwl:id>
        <rdfs:label>Jelnita</rdfs:label>
    </owl:NamedIndividual>
    


    <!-- http://purl.obolibrary.org/obo/GAZ_00368529 -->

    <owl:NamedIndividual rdf:about="http://purl.obolibrary.org/obo/GAZ_00368529">
        <obo:RO_0001025 rdf:resource="http://purl.obolibrary.org/obo/GAZ_00368505"/>
        <obo:IAO_0000115>A river.</obo:IAO_0000115>
        <oboInOwl:hasOBONamespace>GAZ</oboInOwl:hasOBONamespace>
        <oboInOwl:id>GAZ:00368529</oboInOwl:id>
        <rdfs:label>Ghicin</rdfs:label>
    </owl:NamedIndividual>
    


    <!-- http://purl.obolibrary.org/obo/GAZ_00368530 -->

    <owl:NamedIndividual rdf:about="http://purl.obolibrary.org/obo/GAZ_00368530">
        <obo:RO_0001025 rdf:resource="http://purl.obolibrary.org/obo/GAZ_00368505"/>
        <obo:IAO_0000115>A river.</obo:IAO_0000115>
        <oboInOwl:hasOBONamespace>GAZ</oboInOwl:hasOBONamespace>
        <oboInOwl:id>GAZ:00368530</oboInOwl:id>
        <rdfs:label>Vraniu</rdfs:label>
    </owl:NamedIndividual>
    


    <!-- http://purl.obolibrary.org/obo/GAZ_00368531 -->

    <owl:NamedIndividual rdf:about="http://purl.obolibrary.org/obo/GAZ_00368531">
        <obo:RO_0001025 rdf:resource="http://purl.obolibrary.org/obo/GAZ_00368505"/>
        <obo:IAO_0000115>A river.</obo:IAO_0000115>
        <oboInOwl:hasOBONamespace>GAZ</oboInOwl:hasOBONamespace>
        <oboInOwl:id>GAZ:00368531</oboInOwl:id>
        <rdfs:label>Valea Lunga</rdfs:label>
    </owl:NamedIndividual>
    


    <!-- http://purl.obolibrary.org/obo/GAZ_00368532 -->

    <owl:NamedIndividual rdf:about="http://purl.obolibrary.org/obo/GAZ_00368532">
        <obo:IAO_0000115>A river.</obo:IAO_0000115>
        <oboInOwl:hasOBONamespace>GAZ</oboInOwl:hasOBONamespace>
        <oboInOwl:id>GAZ:00368532</oboInOwl:id>
        <rdfs:label>Moscaneasca</rdfs:label>
    </owl:NamedIndividual>
    


    <!-- http://purl.obolibrary.org/obo/GAZ_00368548 -->

    <owl:NamedIndividual rdf:about="http://purl.obolibrary.org/obo/GAZ_00368548">
        <obo:IAO_0000115>A headwater of the Nera River in Romania.</obo:IAO_0000115>
        <oboInOwl:hasOBONamespace>GAZ</oboInOwl:hasOBONamespace>
        <oboInOwl:id>GAZ:00368548</oboInOwl:id>
        <rdfs:label>Nerganita</rdfs:label>
    </owl:NamedIndividual>
    


    <!-- http://purl.obolibrary.org/obo/GAZ_00368550 -->

    <owl:NamedIndividual rdf:about="http://purl.obolibrary.org/obo/GAZ_00368550">
        <obo:IAO_0000115>A river.</obo:IAO_0000115>
        <oboInOwl:hasOBONamespace>GAZ</oboInOwl:hasOBONamespace>
        <oboInOwl:id>GAZ:00368550</oboInOwl:id>
        <rdfs:label>Rudaria</rdfs:label>
    </owl:NamedIndividual>
    


    <!-- http://purl.obolibrary.org/obo/GAZ_00368551 -->

    <owl:NamedIndividual rdf:about="http://purl.obolibrary.org/obo/GAZ_00368551">
        <obo:IAO_0000115>A river.</obo:IAO_0000115>
        <oboInOwl:hasOBONamespace>GAZ</oboInOwl:hasOBONamespace>
        <oboInOwl:id>GAZ:00368551</oboInOwl:id>
        <rdfs:label>Bania</rdfs:label>
    </owl:NamedIndividual>
    


    <!-- http://purl.obolibrary.org/obo/GAZ_00368553 -->

    <owl:NamedIndividual rdf:about="http://purl.obolibrary.org/obo/GAZ_00368553">
        <obo:IAO_0000115>A river.</obo:IAO_0000115>
        <oboInOwl:hasOBONamespace>GAZ</oboInOwl:hasOBONamespace>
        <oboInOwl:id>GAZ:00368553</oboInOwl:id>
        <rdfs:label>Sopotu</rdfs:label>
    </owl:NamedIndividual>
    


    <!-- http://purl.obolibrary.org/obo/GAZ_00368556 -->

    <owl:NamedIndividual rdf:about="http://purl.obolibrary.org/obo/GAZ_00368556">
        <obo:IAO_0000115>A river.</obo:IAO_0000115>
        <oboInOwl:hasOBONamespace>GAZ</oboInOwl:hasOBONamespace>
        <oboInOwl:id>GAZ:00368556</oboInOwl:id>
        <rdfs:label>Rachita</rdfs:label>
    </owl:NamedIndividual>
    


    <!-- http://purl.obolibrary.org/obo/GAZ_00368558 -->

    <owl:NamedIndividual rdf:about="http://purl.obolibrary.org/obo/GAZ_00368558">
        <obo:IAO_0000115>A river.</obo:IAO_0000115>
        <oboInOwl:hasOBONamespace>GAZ</oboInOwl:hasOBONamespace>
        <oboInOwl:id>GAZ:00368558</oboInOwl:id>
        <rdfs:label>Ogasu Babei</rdfs:label>
    </owl:NamedIndividual>
    


    <!-- http://purl.obolibrary.org/obo/GAZ_00368559 -->

    <owl:NamedIndividual rdf:about="http://purl.obolibrary.org/obo/GAZ_00368559">
        <obo:IAO_0000115>A river.</obo:IAO_0000115>
        <oboInOwl:hasOBONamespace>GAZ</oboInOwl:hasOBONamespace>
        <oboInOwl:id>GAZ:00368559</oboInOwl:id>
        <rdfs:label>Ogasu Mare</rdfs:label>
    </owl:NamedIndividual>
    


    <!-- http://purl.obolibrary.org/obo/GAZ_00368560 -->

    <owl:NamedIndividual rdf:about="http://purl.obolibrary.org/obo/GAZ_00368560">
        <obo:IAO_0000115>A river.</obo:IAO_0000115>
        <oboInOwl:hasOBONamespace>GAZ</oboInOwl:hasOBONamespace>
        <oboInOwl:id>GAZ:00368560</oboInOwl:id>
        <rdfs:label>Haimeliug</rdfs:label>
    </owl:NamedIndividual>
    


    <!-- http://purl.obolibrary.org/obo/GAZ_00368561 -->

    <owl:NamedIndividual rdf:about="http://purl.obolibrary.org/obo/GAZ_00368561">
        <obo:IAO_0000115>A river.</obo:IAO_0000115>
        <oboInOwl:hasOBONamespace>GAZ</oboInOwl:hasOBONamespace>
        <oboInOwl:id>GAZ:00368561</oboInOwl:id>
        <rdfs:label>Ogasu Porcului</rdfs:label>
    </owl:NamedIndividual>
    


    <!-- http://purl.obolibrary.org/obo/GAZ_00368562 -->

    <owl:NamedIndividual rdf:about="http://purl.obolibrary.org/obo/GAZ_00368562">
        <obo:IAO_0000115>A river.</obo:IAO_0000115>
        <oboInOwl:hasOBONamespace>GAZ</oboInOwl:hasOBONamespace>
        <oboInOwl:id>GAZ:00368562</oboInOwl:id>
        <rdfs:label>Ulmu Mic</rdfs:label>
    </owl:NamedIndividual>
    


    <!-- http://purl.obolibrary.org/obo/GAZ_00368563 -->

    <owl:NamedIndividual rdf:about="http://purl.obolibrary.org/obo/GAZ_00368563">
        <obo:IAO_0000115>A river.</obo:IAO_0000115>
        <oboInOwl:hasOBONamespace>GAZ</oboInOwl:hasOBONamespace>
        <oboInOwl:id>GAZ:00368563</oboInOwl:id>
        <rdfs:label>Ulmu Mare</rdfs:label>
    </owl:NamedIndividual>
    


    <!-- http://purl.obolibrary.org/obo/GAZ_00368565 -->

    <owl:NamedIndividual rdf:about="http://purl.obolibrary.org/obo/GAZ_00368565">
        <obo:IAO_0000115>A river.</obo:IAO_0000115>
        <oboInOwl:hasOBONamespace>GAZ</oboInOwl:hasOBONamespace>
        <oboInOwl:id>GAZ:00368565</oboInOwl:id>
        <rdfs:label>Padina Baschii</rdfs:label>
    </owl:NamedIndividual>
    


    <!-- http://purl.obolibrary.org/obo/GAZ_00368566 -->

    <owl:NamedIndividual rdf:about="http://purl.obolibrary.org/obo/GAZ_00368566">
        <obo:IAO_0000115>A river.</obo:IAO_0000115>
        <oboInOwl:hasOBONamespace>GAZ</oboInOwl:hasOBONamespace>
        <oboInOwl:id>GAZ:00368566</oboInOwl:id>
        <rdfs:label>Susara</rdfs:label>
    </owl:NamedIndividual>
    


    <!-- http://purl.obolibrary.org/obo/GAZ_00368567 -->

    <owl:NamedIndividual rdf:about="http://purl.obolibrary.org/obo/GAZ_00368567">
        <obo:IAO_0000115>A river.</obo:IAO_0000115>
        <oboInOwl:hasOBONamespace>GAZ</oboInOwl:hasOBONamespace>
        <oboInOwl:id>GAZ:00368567</oboInOwl:id>
        <rdfs:label>Fantana Seaca</rdfs:label>
    </owl:NamedIndividual>
    


    <!-- http://purl.obolibrary.org/obo/GAZ_00368568 -->

    <owl:NamedIndividual rdf:about="http://purl.obolibrary.org/obo/GAZ_00368568">
        <obo:IAO_0000115>A headwater of the Nera River in Romania.</obo:IAO_0000115>
        <oboInOwl:hasOBONamespace>GAZ</oboInOwl:hasOBONamespace>
        <oboInOwl:id>GAZ:00368568</oboInOwl:id>
        <rdfs:label>Nergana</rdfs:label>
    </owl:NamedIndividual>
    


    <!-- http://purl.obolibrary.org/obo/GAZ_00368569 -->

    <owl:NamedIndividual rdf:about="http://purl.obolibrary.org/obo/GAZ_00368569">
        <obo:IAO_0000115>A river.</obo:IAO_0000115>
        <oboInOwl:hasOBONamespace>GAZ</oboInOwl:hasOBONamespace>
        <oboInOwl:id>GAZ:00368569</oboInOwl:id>
        <rdfs:label>Cosava</rdfs:label>
    </owl:NamedIndividual>
    


    <!-- http://purl.obolibrary.org/obo/GAZ_00368570 -->

    <owl:NamedIndividual rdf:about="http://purl.obolibrary.org/obo/GAZ_00368570">
        <obo:IAO_0000115>A river.</obo:IAO_0000115>
        <oboInOwl:hasOBONamespace>GAZ</oboInOwl:hasOBONamespace>
        <oboInOwl:id>GAZ:00368570</oboInOwl:id>
        <rdfs:label>Hiclisag</rdfs:label>
    </owl:NamedIndividual>
    


    <!-- http://purl.obolibrary.org/obo/GAZ_00368573 -->

    <owl:NamedIndividual rdf:about="http://purl.obolibrary.org/obo/GAZ_00368573">
        <obo:IAO_0000115>A river.</obo:IAO_0000115>
        <oboInOwl:hasOBONamespace>GAZ</oboInOwl:hasOBONamespace>
        <oboInOwl:id>GAZ:00368573</oboInOwl:id>
        <rdfs:label>Agris</rdfs:label>
    </owl:NamedIndividual>
    


    <!-- http://purl.obolibrary.org/obo/GAZ_00368574 -->

    <owl:NamedIndividual rdf:about="http://purl.obolibrary.org/obo/GAZ_00368574">
        <obo:IAO_0000115>A river.</obo:IAO_0000115>
        <oboInOwl:hasOBONamespace>GAZ</oboInOwl:hasOBONamespace>
        <oboInOwl:id>GAZ:00368574</oboInOwl:id>
        <rdfs:label>Lapusnicu</rdfs:label>
    </owl:NamedIndividual>
    


    <!-- http://purl.obolibrary.org/obo/GAZ_00368575 -->

    <owl:NamedIndividual rdf:about="http://purl.obolibrary.org/obo/GAZ_00368575">
        <obo:IAO_0000115>A river.</obo:IAO_0000115>
        <oboInOwl:hasOBONamespace>GAZ</oboInOwl:hasOBONamespace>
        <oboInOwl:id>GAZ:00368575</oboInOwl:id>
        <rdfs:label>Orestica</rdfs:label>
    </owl:NamedIndividual>
    


    <!-- http://purl.obolibrary.org/obo/GAZ_00368576 -->

    <owl:NamedIndividual rdf:about="http://purl.obolibrary.org/obo/GAZ_00368576">
        <obo:IAO_0000115>A river.</obo:IAO_0000115>
        <oboInOwl:hasOBONamespace>GAZ</oboInOwl:hasOBONamespace>
        <oboInOwl:id>GAZ:00368576</oboInOwl:id>
        <rdfs:label>Moceris</rdfs:label>
    </owl:NamedIndividual>
    


    <!-- http://purl.obolibrary.org/obo/GAZ_00368577 -->

    <owl:NamedIndividual rdf:about="http://purl.obolibrary.org/obo/GAZ_00368577">
        <obo:IAO_0000115>A river.</obo:IAO_0000115>
        <oboInOwl:hasOBONamespace>GAZ</oboInOwl:hasOBONamespace>
        <oboInOwl:id>GAZ:00368577</oboInOwl:id>
        <rdfs:label>Ducin</rdfs:label>
    </owl:NamedIndividual>
    


    <!-- http://purl.obolibrary.org/obo/GAZ_00368578 -->

    <owl:NamedIndividual rdf:about="http://purl.obolibrary.org/obo/GAZ_00368578">
        <obo:IAO_0000115>A river.</obo:IAO_0000115>
        <oboInOwl:hasOBONamespace>GAZ</oboInOwl:hasOBONamespace>
        <oboInOwl:id>GAZ:00368578</oboInOwl:id>
        <rdfs:label>Bresnic</rdfs:label>
    </owl:NamedIndividual>
    


    <!-- http://purl.obolibrary.org/obo/GAZ_00368579 -->

    <owl:NamedIndividual rdf:about="http://purl.obolibrary.org/obo/GAZ_00368579">
        <obo:IAO_0000115>A river.</obo:IAO_0000115>
        <oboInOwl:hasOBONamespace>GAZ</oboInOwl:hasOBONamespace>
        <oboInOwl:id>GAZ:00368579</oboInOwl:id>
        <rdfs:label>Arsa</rdfs:label>
    </owl:NamedIndividual>
    


    <!-- http://purl.obolibrary.org/obo/GAZ_00368580 -->

    <owl:NamedIndividual rdf:about="http://purl.obolibrary.org/obo/GAZ_00368580">
        <obo:IAO_0000115>A river.</obo:IAO_0000115>
        <oboInOwl:hasOBONamespace>GAZ</oboInOwl:hasOBONamespace>
        <oboInOwl:id>GAZ:00368580</oboInOwl:id>
        <rdfs:label>Meliugel</rdfs:label>
    </owl:NamedIndividual>
    


    <!-- http://purl.obolibrary.org/obo/GAZ_00368581 -->

    <owl:NamedIndividual rdf:about="http://purl.obolibrary.org/obo/GAZ_00368581">
        <obo:IAO_0000115>A river.</obo:IAO_0000115>
        <oboInOwl:hasOBONamespace>GAZ</oboInOwl:hasOBONamespace>
        <oboInOwl:id>GAZ:00368581</oboInOwl:id>
        <rdfs:label>Raul Dracului</rdfs:label>
    </owl:NamedIndividual>
    


    <!-- http://purl.obolibrary.org/obo/GAZ_00368582 -->

    <owl:NamedIndividual rdf:about="http://purl.obolibrary.org/obo/GAZ_00368582">
        <obo:IAO_0000115>A river.</obo:IAO_0000115>
        <oboInOwl:hasOBONamespace>GAZ</oboInOwl:hasOBONamespace>
        <oboInOwl:id>GAZ:00368582</oboInOwl:id>
        <rdfs:label>Ogasu Alunilor</rdfs:label>
    </owl:NamedIndividual>
    


    <!-- http://purl.obolibrary.org/obo/GAZ_00368583 -->

    <owl:NamedIndividual rdf:about="http://purl.obolibrary.org/obo/GAZ_00368583">
        <obo:IAO_0000115>A river.</obo:IAO_0000115>
        <oboInOwl:hasOBONamespace>GAZ</oboInOwl:hasOBONamespace>
        <oboInOwl:id>GAZ:00368583</oboInOwl:id>
        <rdfs:label>Radovanu</rdfs:label>
    </owl:NamedIndividual>
    


    <!-- http://purl.obolibrary.org/obo/GAZ_00368584 -->

    <owl:NamedIndividual rdf:about="http://purl.obolibrary.org/obo/GAZ_00368584">
        <obo:IAO_0000115>A river.</obo:IAO_0000115>
        <oboInOwl:hasOBONamespace>GAZ</oboInOwl:hasOBONamespace>
        <oboInOwl:id>GAZ:00368584</oboInOwl:id>
        <rdfs:label>Valea Rea</rdfs:label>
    </owl:NamedIndividual>
    


    <!-- http://purl.obolibrary.org/obo/GAZ_00368586 -->

    <owl:NamedIndividual rdf:about="http://purl.obolibrary.org/obo/GAZ_00368586">
        <obo:IAO_0000115>A river.</obo:IAO_0000115>
        <oboInOwl:hasOBONamespace>GAZ</oboInOwl:hasOBONamespace>
        <oboInOwl:id>GAZ:00368586</oboInOwl:id>
        <rdfs:label>Lindina</rdfs:label>
    </owl:NamedIndividual>
    


    <!-- http://purl.obolibrary.org/obo/GAZ_00368587 -->

    <owl:NamedIndividual rdf:about="http://purl.obolibrary.org/obo/GAZ_00368587">
        <obo:IAO_0000115>A river.</obo:IAO_0000115>
        <oboInOwl:hasOBONamespace>GAZ</oboInOwl:hasOBONamespace>
        <oboInOwl:id>GAZ:00368587</oboInOwl:id>
        <rdfs:label>Beu</rdfs:label>
    </owl:NamedIndividual>
    


    <!-- http://purl.obolibrary.org/obo/GAZ_00368600 -->

    <owl:NamedIndividual rdf:about="http://purl.obolibrary.org/obo/GAZ_00368600">
        <obo:IAO_0000115>A river.</obo:IAO_0000115>
        <oboInOwl:hasOBONamespace>GAZ</oboInOwl:hasOBONamespace>
        <oboInOwl:id>GAZ:00368600</oboInOwl:id>
        <rdfs:label>Ciurezu</rdfs:label>
    </owl:NamedIndividual>
    


    <!-- http://purl.obolibrary.org/obo/GAZ_00368602 -->

    <owl:NamedIndividual rdf:about="http://purl.obolibrary.org/obo/GAZ_00368602">
        <obo:IAO_0000115>A river. It joins the Minis through a system of caves.</obo:IAO_0000115>
        <oboInOwl:hasOBONamespace>GAZ</oboInOwl:hasOBONamespace>
        <oboInOwl:id>GAZ:00368602</oboInOwl:id>
        <rdfs:label>Ponor</rdfs:label>
    </owl:NamedIndividual>
    


    <!-- http://purl.obolibrary.org/obo/GAZ_00368603 -->

    <owl:NamedIndividual rdf:about="http://purl.obolibrary.org/obo/GAZ_00368603">
        <obo:IAO_0000115>A river.</obo:IAO_0000115>
        <oboInOwl:hasOBONamespace>GAZ</oboInOwl:hasOBONamespace>
        <oboInOwl:id>GAZ:00368603</oboInOwl:id>
        <rdfs:label>Predilcova</rdfs:label>
    </owl:NamedIndividual>
    


    <!-- http://purl.obolibrary.org/obo/GAZ_00368604 -->

    <owl:NamedIndividual rdf:about="http://purl.obolibrary.org/obo/GAZ_00368604">
        <obo:IAO_0000115>A river.</obo:IAO_0000115>
        <oboInOwl:hasOBONamespace>GAZ</oboInOwl:hasOBONamespace>
        <oboInOwl:id>GAZ:00368604</oboInOwl:id>
        <rdfs:label>Marasca</rdfs:label>
    </owl:NamedIndividual>
    


    <!-- http://purl.obolibrary.org/obo/GAZ_00368605 -->

    <owl:NamedIndividual rdf:about="http://purl.obolibrary.org/obo/GAZ_00368605">
        <obo:IAO_0000115>A river.</obo:IAO_0000115>
        <oboInOwl:hasOBONamespace>GAZ</oboInOwl:hasOBONamespace>
        <oboInOwl:id>GAZ:00368605</oboInOwl:id>
        <rdfs:label>Ogasu Babei</rdfs:label>
    </owl:NamedIndividual>
    


    <!-- http://purl.obolibrary.org/obo/GAZ_00368606 -->

    <owl:NamedIndividual rdf:about="http://purl.obolibrary.org/obo/GAZ_00368606">
        <obo:IAO_0000115>A river.</obo:IAO_0000115>
        <oboInOwl:hasOBONamespace>GAZ</oboInOwl:hasOBONamespace>
        <oboInOwl:id>GAZ:00368606</oboInOwl:id>
        <rdfs:label>Ogasu Mare</rdfs:label>
    </owl:NamedIndividual>
    


    <!-- http://purl.obolibrary.org/obo/GAZ_00368607 -->

    <owl:NamedIndividual rdf:about="http://purl.obolibrary.org/obo/GAZ_00368607">
        <obo:IAO_0000115>A river.</obo:IAO_0000115>
        <oboInOwl:hasOBONamespace>GAZ</oboInOwl:hasOBONamespace>
        <oboInOwl:id>GAZ:00368607</oboInOwl:id>
        <rdfs:label>Poneasca</rdfs:label>
    </owl:NamedIndividual>
    


    <!-- http://purl.obolibrary.org/obo/GAZ_00368608 -->

    <owl:NamedIndividual rdf:about="http://purl.obolibrary.org/obo/GAZ_00368608">
        <obo:IAO_0000115>A river.</obo:IAO_0000115>
        <oboInOwl:hasOBONamespace>GAZ</oboInOwl:hasOBONamespace>
        <oboInOwl:id>GAZ:00368608</oboInOwl:id>
        <rdfs:label>Zagraza</rdfs:label>
    </owl:NamedIndividual>
    


    <!-- http://purl.obolibrary.org/obo/GAZ_00368609 -->

    <owl:NamedIndividual rdf:about="http://purl.obolibrary.org/obo/GAZ_00368609">
        <obo:IAO_0000115>A river.</obo:IAO_0000115>
        <oboInOwl:hasOBONamespace>GAZ</oboInOwl:hasOBONamespace>
        <oboInOwl:id>GAZ:00368609</oboInOwl:id>
        <rdfs:label>Taria</rdfs:label>
    </owl:NamedIndividual>
    


    <!-- http://purl.obolibrary.org/obo/GAZ_00368610 -->

    <owl:NamedIndividual rdf:about="http://purl.obolibrary.org/obo/GAZ_00368610">
        <obo:IAO_0000115>A river.</obo:IAO_0000115>
        <oboInOwl:hasOBONamespace>GAZ</oboInOwl:hasOBONamespace>
        <oboInOwl:id>GAZ:00368610</oboInOwl:id>
        <rdfs:label>Mandrisag</rdfs:label>
    </owl:NamedIndividual>
    


    <!-- http://purl.obolibrary.org/obo/GAZ_00368611 -->

    <owl:NamedIndividual rdf:about="http://purl.obolibrary.org/obo/GAZ_00368611">
        <obo:IAO_0000115>A river.</obo:IAO_0000115>
        <oboInOwl:hasOBONamespace>GAZ</oboInOwl:hasOBONamespace>
        <oboInOwl:id>GAZ:00368611</oboInOwl:id>
        <rdfs:label>Calugaru</rdfs:label>
    </owl:NamedIndividual>
    


    <!-- http://purl.obolibrary.org/obo/GAZ_00368612 -->

    <owl:NamedIndividual rdf:about="http://purl.obolibrary.org/obo/GAZ_00368612">
        <obo:IAO_0000115>A river.</obo:IAO_0000115>
        <oboInOwl:hasOBONamespace>GAZ</oboInOwl:hasOBONamespace>
        <oboInOwl:id>GAZ:00368612</oboInOwl:id>
        <rdfs:label>Pauleasca</rdfs:label>
    </owl:NamedIndividual>
    


    <!-- http://purl.obolibrary.org/obo/GAZ_00368613 -->

    <owl:NamedIndividual rdf:about="http://purl.obolibrary.org/obo/GAZ_00368613">
        <obo:IAO_0000115>A river.</obo:IAO_0000115>
        <oboInOwl:hasOBONamespace>GAZ</oboInOwl:hasOBONamespace>
        <oboInOwl:id>GAZ:00368613</oboInOwl:id>
        <rdfs:label>Golumbu</rdfs:label>
    </owl:NamedIndividual>
    


    <!-- http://purl.obolibrary.org/obo/GAZ_00368614 -->

    <owl:NamedIndividual rdf:about="http://purl.obolibrary.org/obo/GAZ_00368614">
        <obo:IAO_0000115>A river.</obo:IAO_0000115>
        <oboInOwl:hasOBONamespace>GAZ</oboInOwl:hasOBONamespace>
        <oboInOwl:id>GAZ:00368614</oboInOwl:id>
        <rdfs:label>Valea Maraetilor</rdfs:label>
    </owl:NamedIndividual>
    


    <!-- http://purl.obolibrary.org/obo/GAZ_00368615 -->

    <owl:NamedIndividual rdf:about="http://purl.obolibrary.org/obo/GAZ_00368615">
        <obo:IAO_0000115>A river.</obo:IAO_0000115>
        <oboInOwl:hasOBONamespace>GAZ</oboInOwl:hasOBONamespace>
        <oboInOwl:id>GAZ:00368615</oboInOwl:id>
        <rdfs:label>Bozovici</rdfs:label>
    </owl:NamedIndividual>
    


    <!-- http://purl.obolibrary.org/obo/GAZ_00368617 -->

    <owl:NamedIndividual rdf:about="http://purl.obolibrary.org/obo/GAZ_00368617">
        <obo:IAO_0000115>A river.</obo:IAO_0000115>
        <oboInOwl:hasOBONamespace>GAZ</oboInOwl:hasOBONamespace>
        <oboInOwl:id>GAZ:00368617</oboInOwl:id>
        <rdfs:label>Ogasu Bologhii</rdfs:label>
    </owl:NamedIndividual>
    


    <!-- http://purl.obolibrary.org/obo/GAZ_00368618 -->

    <owl:NamedIndividual rdf:about="http://purl.obolibrary.org/obo/GAZ_00368618">
        <obo:IAO_0000115>A river.</obo:IAO_0000115>
        <oboInOwl:hasOBONamespace>GAZ</oboInOwl:hasOBONamespace>
        <oboInOwl:id>GAZ:00368618</oboInOwl:id>
        <rdfs:label>Gusec</rdfs:label>
    </owl:NamedIndividual>
    


    <!-- http://purl.obolibrary.org/obo/GAZ_00368619 -->

    <owl:NamedIndividual rdf:about="http://purl.obolibrary.org/obo/GAZ_00368619">
        <obo:IAO_0000115>A river.</obo:IAO_0000115>
        <oboInOwl:hasOBONamespace>GAZ</oboInOwl:hasOBONamespace>
        <oboInOwl:id>GAZ:00368619</oboInOwl:id>
        <rdfs:label>Ogasu cu Raci</rdfs:label>
    </owl:NamedIndividual>
    


    <!-- http://purl.obolibrary.org/obo/GAZ_00368620 -->

    <owl:NamedIndividual rdf:about="http://purl.obolibrary.org/obo/GAZ_00368620">
        <obo:IAO_0000115>A river.</obo:IAO_0000115>
        <oboInOwl:hasOBONamespace>GAZ</oboInOwl:hasOBONamespace>
        <oboInOwl:id>GAZ:00368620</oboInOwl:id>
        <rdfs:label>Prisaca</rdfs:label>
    </owl:NamedIndividual>
    


    <!-- http://purl.obolibrary.org/obo/GAZ_00368621 -->

    <owl:NamedIndividual rdf:about="http://purl.obolibrary.org/obo/GAZ_00368621">
        <obo:IAO_0000115>A river.</obo:IAO_0000115>
        <oboInOwl:hasOBONamespace>GAZ</oboInOwl:hasOBONamespace>
        <oboInOwl:id>GAZ:00368621</oboInOwl:id>
        <rdfs:label>Valaul Coziei</rdfs:label>
    </owl:NamedIndividual>
    


    <!-- http://purl.obolibrary.org/obo/GAZ_00368622 -->

    <owl:NamedIndividual rdf:about="http://purl.obolibrary.org/obo/GAZ_00368622">
        <obo:IAO_0000115>A river.</obo:IAO_0000115>
        <oboInOwl:hasOBONamespace>GAZ</oboInOwl:hasOBONamespace>
        <oboInOwl:id>GAZ:00368622</oboInOwl:id>
        <rdfs:label>Padina Brata</rdfs:label>
    </owl:NamedIndividual>
    


    <!-- http://purl.obolibrary.org/obo/GAZ_00368623 -->

    <owl:NamedIndividual rdf:about="http://purl.obolibrary.org/obo/GAZ_00368623">
        <obo:IAO_0000115>A river.</obo:IAO_0000115>
        <oboInOwl:hasOBONamespace>GAZ</oboInOwl:hasOBONamespace>
        <oboInOwl:id>GAZ:00368623</oboInOwl:id>
        <rdfs:label>Padina Seaca</rdfs:label>
    </owl:NamedIndividual>
    


    <!-- http://purl.obolibrary.org/obo/GAZ_00368629 -->

    <owl:NamedIndividual rdf:about="http://purl.obolibrary.org/obo/GAZ_00368629">
        <obo:IAO_0000115>A river.</obo:IAO_0000115>
        <oboInOwl:hasOBONamespace>GAZ</oboInOwl:hasOBONamespace>
        <oboInOwl:id>GAZ:00368629</oboInOwl:id>
        <rdfs:label>Blezniac</rdfs:label>
    </owl:NamedIndividual>
    


    <!-- http://purl.obolibrary.org/obo/GAZ_00368636 -->

    <owl:NamedIndividual rdf:about="http://purl.obolibrary.org/obo/GAZ_00368636">
        <obo:IAO_0000115>A man-made island Formed in 1909 with the construction of the Mohovo-Sarengrad canal. Claimed by Croatia and Serbia.</obo:IAO_0000115>
        <oboInOwl:hasOBONamespace>GAZ</oboInOwl:hasOBONamespace>
        <oboInOwl:id>GAZ:00368636</oboInOwl:id>
        <rdfs:label>Sarengradska ada</rdfs:label>
    </owl:NamedIndividual>
    


    <!-- http://purl.obolibrary.org/obo/GAZ_00368637 -->

    <owl:NamedIndividual rdf:about="http://purl.obolibrary.org/obo/GAZ_00368637">
        <obo:IAO_0000115>An island. Claimed by Serbia.</obo:IAO_0000115>
        <oboInOwl:hasOBONamespace>GAZ</oboInOwl:hasOBONamespace>
        <oboInOwl:id>GAZ:00368637</oboInOwl:id>
        <rdfs:label>Vukovarska ada</rdfs:label>
    </owl:NamedIndividual>
    


    <!-- http://purl.obolibrary.org/obo/GAZ_00368641 -->

    <owl:NamedIndividual rdf:about="http://purl.obolibrary.org/obo/GAZ_00368641">
        <obo:RO_0001025 rdf:resource="http://purl.obolibrary.org/obo/GAZ_00014333"/>
        <obo:IAO_0000115>A populated place.</obo:IAO_0000115>
        <oboInOwl:hasOBONamespace>GAZ</oboInOwl:hasOBONamespace>
        <oboInOwl:id>GAZ:00368641</oboInOwl:id>
        <rdfs:label>Felsoszentivan</rdfs:label>
    </owl:NamedIndividual>
    


    <!-- http://purl.obolibrary.org/obo/GAZ_00368642 -->

    <owl:NamedIndividual rdf:about="http://purl.obolibrary.org/obo/GAZ_00368642">
        <obo:RO_0001025 rdf:resource="http://purl.obolibrary.org/obo/GAZ_00014333"/>
        <obo:IAO_0000115>A populated place.</obo:IAO_0000115>
        <oboInOwl:hasOBONamespace>GAZ</oboInOwl:hasOBONamespace>
        <oboInOwl:id>GAZ:00368642</oboInOwl:id>
        <rdfs:label>Bacsbokod</rdfs:label>
    </owl:NamedIndividual>
    


    <!-- http://purl.obolibrary.org/obo/GAZ_00368643 -->

    <owl:NamedIndividual rdf:about="http://purl.obolibrary.org/obo/GAZ_00368643">
        <obo:RO_0001025 rdf:resource="http://purl.obolibrary.org/obo/GAZ_00014333"/>
        <obo:IAO_0000115>A populated place.</obo:IAO_0000115>
        <oboInOwl:hasOBONamespace>GAZ</oboInOwl:hasOBONamespace>
        <oboInOwl:id>GAZ:00368643</oboInOwl:id>
        <rdfs:label>Bacsborsod</rdfs:label>
    </owl:NamedIndividual>
    


    <!-- http://purl.obolibrary.org/obo/GAZ_00368644 -->

    <owl:NamedIndividual rdf:about="http://purl.obolibrary.org/obo/GAZ_00368644">
        <obo:RO_0001025 rdf:resource="http://purl.obolibrary.org/obo/GAZ_00014333"/>
        <obo:IAO_0000115>A populated place.</obo:IAO_0000115>
        <oboInOwl:hasOBONamespace>GAZ</oboInOwl:hasOBONamespace>
        <oboInOwl:id>GAZ:00368644</oboInOwl:id>
        <rdfs:label>Tatahaza</rdfs:label>
    </owl:NamedIndividual>
    


    <!-- http://purl.obolibrary.org/obo/GAZ_00368645 -->

    <owl:NamedIndividual rdf:about="http://purl.obolibrary.org/obo/GAZ_00368645">
        <obo:RO_0001025 rdf:resource="http://purl.obolibrary.org/obo/GAZ_00014333"/>
        <obo:IAO_0000115>A populated place.</obo:IAO_0000115>
        <oboInOwl:hasOBONamespace>GAZ</oboInOwl:hasOBONamespace>
        <oboInOwl:id>GAZ:00368645</oboInOwl:id>
        <rdfs:label>Matetelke</rdfs:label>
    </owl:NamedIndividual>
    


    <!-- http://purl.obolibrary.org/obo/GAZ_00368646 -->

    <owl:NamedIndividual rdf:about="http://purl.obolibrary.org/obo/GAZ_00368646">
        <obo:RO_0001025 rdf:resource="http://purl.obolibrary.org/obo/GAZ_00014333"/>
        <obo:IAO_0000115>A populated place.</obo:IAO_0000115>
        <oboInOwl:hasOBONamespace>GAZ</oboInOwl:hasOBONamespace>
        <oboInOwl:id>GAZ:00368646</oboInOwl:id>
        <rdfs:label>Katymar</rdfs:label>
    </owl:NamedIndividual>
    


    <!-- http://purl.obolibrary.org/obo/GAZ_00368650 -->

    <owl:NamedIndividual rdf:about="http://purl.obolibrary.org/obo/GAZ_00368650">
        <obo:IAO_0000115>An island formed where the Nadela enters the Danube.</obo:IAO_0000115>
        <oboInOwl:hasOBONamespace>GAZ</oboInOwl:hasOBONamespace>
        <oboInOwl:id>GAZ:00368650</oboInOwl:id>
        <rdfs:label>Vanovo Ostrvo</rdfs:label>
    </owl:NamedIndividual>
    


    <!-- http://purl.obolibrary.org/obo/GAZ_00368677 -->

    <owl:NamedIndividual rdf:about="http://purl.obolibrary.org/obo/GAZ_00368677">
        <obo:RO_0001025 rdf:resource="http://purl.obolibrary.org/obo/GAZ_00062794"/>
        <obo:IAO_0000115>A man-made lake.</obo:IAO_0000115>
        <oboInOwl:hasOBONamespace>GAZ</oboInOwl:hasOBONamespace>
        <oboInOwl:id>GAZ:00368677</oboInOwl:id>
        <rdfs:label>Radoinja Lake</rdfs:label>
    </owl:NamedIndividual>
    


    <!-- http://purl.obolibrary.org/obo/GAZ_00368680 -->

    <owl:NamedIndividual rdf:about="http://purl.obolibrary.org/obo/GAZ_00368680">
        <obo:IAO_0000115>A man-made reservoir.</obo:IAO_0000115>
        <oboInOwl:hasOBONamespace>GAZ</oboInOwl:hasOBONamespace>
        <oboInOwl:id>GAZ:00368680</oboInOwl:id>
        <rdfs:label>Vrutci Lake</rdfs:label>
    </owl:NamedIndividual>
    


    <!-- http://purl.obolibrary.org/obo/GAZ_00368694 -->

    <owl:NamedIndividual rdf:about="http://purl.obolibrary.org/obo/GAZ_00368694">
        <obo:IAO_0000115>A headwater of the Pek.</obo:IAO_0000115>
        <oboInOwl:hasOBONamespace>GAZ</oboInOwl:hasOBONamespace>
        <oboInOwl:id>GAZ:00368694</oboInOwl:id>
        <rdfs:label>Veliki Pek</rdfs:label>
    </owl:NamedIndividual>
    


    <!-- http://purl.obolibrary.org/obo/GAZ_00368695 -->

    <owl:NamedIndividual rdf:about="http://purl.obolibrary.org/obo/GAZ_00368695">
        <obo:IAO_0000115>A headwater of the Pek.</obo:IAO_0000115>
        <oboInOwl:hasOBONamespace>GAZ</oboInOwl:hasOBONamespace>
        <oboInOwl:id>GAZ:00368695</oboInOwl:id>
        <rdfs:label>Mali Pek</rdfs:label>
    </owl:NamedIndividual>
    


    <!-- http://purl.obolibrary.org/obo/GAZ_00368724 -->

    <owl:NamedIndividual rdf:about="http://purl.obolibrary.org/obo/GAZ_00368724">
        <obo:IAO_0000115>A river in eastern Serbia and western Bulgaria.</obo:IAO_0000115>
        <oboInOwl:hasOBONamespace>GAZ</oboInOwl:hasOBONamespace>
        <oboInOwl:id>GAZ:00368724</oboInOwl:id>
        <rdfs:label>Timok</rdfs:label>
    </owl:NamedIndividual>
    


    <!-- http://purl.obolibrary.org/obo/GAZ_00368807 -->

    <owl:NamedIndividual rdf:about="http://purl.obolibrary.org/obo/GAZ_00368807">
        <obo:IAO_0000115>An island.</obo:IAO_0000115>
        <oboInOwl:hasOBONamespace>GAZ</oboInOwl:hasOBONamespace>
        <oboInOwl:id>GAZ:00368807</oboInOwl:id>
        <rdfs:label>Biserno Ostrvo</rdfs:label>
    </owl:NamedIndividual>
    


    <!-- http://purl.obolibrary.org/obo/GAZ_00368808 -->

    <owl:NamedIndividual rdf:about="http://purl.obolibrary.org/obo/GAZ_00368808">
        <obo:IAO_0000115>An island.</obo:IAO_0000115>
        <oboInOwl:hasOBONamespace>GAZ</oboInOwl:hasOBONamespace>
        <oboInOwl:id>GAZ:00368808</oboInOwl:id>
        <rdfs:label>Krcedinska ada</rdfs:label>
    </owl:NamedIndividual>
    


    <!-- http://purl.obolibrary.org/obo/GAZ_00369492 -->

    <owl:NamedIndividual rdf:about="http://purl.obolibrary.org/obo/GAZ_00369492">
        <obo:IAO_0000115>A lake.</obo:IAO_0000115>
        <oboInOwl:hasOBONamespace>GAZ</oboInOwl:hasOBONamespace>
        <oboInOwl:id>GAZ:00369492</oboInOwl:id>
        <rdfs:label>Veliko Plivsko Lake</rdfs:label>
    </owl:NamedIndividual>
    


    <!-- http://purl.obolibrary.org/obo/GAZ_00369493 -->

    <owl:NamedIndividual rdf:about="http://purl.obolibrary.org/obo/GAZ_00369493">
        <obo:IAO_0000115>A lake.</obo:IAO_0000115>
        <oboInOwl:hasOBONamespace>GAZ</oboInOwl:hasOBONamespace>
        <oboInOwl:id>GAZ:00369493</oboInOwl:id>
        <rdfs:label>Malo Plivsko Lake</rdfs:label>
    </owl:NamedIndividual>
    


    <!-- http://purl.obolibrary.org/obo/GAZ_00369494 -->

    <owl:NamedIndividual rdf:about="http://purl.obolibrary.org/obo/GAZ_00369494">
        <obo:IAO_0000115>A lake.</obo:IAO_0000115>
        <oboInOwl:hasOBONamespace>GAZ</oboInOwl:hasOBONamespace>
        <oboInOwl:id>GAZ:00369494</oboInOwl:id>
        <rdfs:label>Okruglo Lake</rdfs:label>
    </owl:NamedIndividual>
    


    <!-- http://purl.obolibrary.org/obo/GAZ_00372039 -->

    <owl:NamedIndividual rdf:about="http://purl.obolibrary.org/obo/GAZ_00372039">
        <obo:IAO_0000115>A hydroelectric power plant.</obo:IAO_0000115>
        <oboInOwl:hasOBONamespace>GAZ</oboInOwl:hasOBONamespace>
        <oboInOwl:id>GAZ:00372039</oboInOwl:id>
        <rdfs:label>Gojak Hydroelectric Power Plant</rdfs:label>
    </owl:NamedIndividual>
    


    <!-- http://purl.obolibrary.org/obo/GAZ_00372040 -->

    <owl:NamedIndividual rdf:about="http://purl.obolibrary.org/obo/GAZ_00372040">
        <obo:IAO_0000115>A hydroelectric power plant.</obo:IAO_0000115>
        <oboInOwl:hasOBONamespace>GAZ</oboInOwl:hasOBONamespace>
        <oboInOwl:id>GAZ:00372040</oboInOwl:id>
        <rdfs:label>Ozalj Hydroelectric Power Plant</rdfs:label>
    </owl:NamedIndividual>
    


    <!-- http://purl.obolibrary.org/obo/GAZ_00372043 -->

    <owl:NamedIndividual rdf:about="http://purl.obolibrary.org/obo/GAZ_00372043">
        <obo:IAO_0000115>A hydroelectric power plant.</obo:IAO_0000115>
        <oboInOwl:hasOBONamespace>GAZ</oboInOwl:hasOBONamespace>
        <oboInOwl:id>GAZ:00372043</oboInOwl:id>
        <rdfs:label>Varazdin Hydroelectric Power Plant</rdfs:label>
    </owl:NamedIndividual>
    


    <!-- http://purl.obolibrary.org/obo/GAZ_00372044 -->

    <owl:NamedIndividual rdf:about="http://purl.obolibrary.org/obo/GAZ_00372044">
        <obo:IAO_0000115>A lake.</obo:IAO_0000115>
        <oboInOwl:hasOBONamespace>GAZ</oboInOwl:hasOBONamespace>
        <oboInOwl:id>GAZ:00372044</oboInOwl:id>
        <rdfs:label>Soderica</rdfs:label>
    </owl:NamedIndividual>
    


    <!-- http://purl.obolibrary.org/obo/GAZ_00372083 -->

    <owl:NamedIndividual rdf:about="http://purl.obolibrary.org/obo/GAZ_00372083">
        <obo:IAO_0000115>A hydroelectric power plant on river Krka, located in Sibenik-Knin county.</obo:IAO_0000115>
        <oboInOwl:hasOBONamespace>GAZ</oboInOwl:hasOBONamespace>
        <oboInOwl:id>GAZ:00372083</oboInOwl:id>
        <rdfs:label>Jaruga Hydroelectric Power Plant</rdfs:label>
    </owl:NamedIndividual>
    


    <!-- http://purl.obolibrary.org/obo/GAZ_00372093 -->

    <owl:NamedIndividual rdf:about="http://purl.obolibrary.org/obo/GAZ_00372093">
        <obo:IAO_0000115>A lake near the city of Skradin in the Croatian region of Dalmatia. It is not entirely closed, but is connected to the sea by a narrow channel which leads to Sibenik harbor.</obo:IAO_0000115>
        <oboInOwl:hasOBONamespace>GAZ</oboInOwl:hasOBONamespace>
        <oboInOwl:id>GAZ:00372093</oboInOwl:id>
        <rdfs:label>Prokljansko jezero</rdfs:label>
    </owl:NamedIndividual>
    


    <!-- http://purl.obolibrary.org/obo/GAZ_00372094 -->

    <owl:NamedIndividual rdf:about="http://purl.obolibrary.org/obo/GAZ_00372094">
        <obo:IAO_0000115>A hydroelectric power plant. Located located 7 km north of the town of Knin, in Golubic village.</obo:IAO_0000115>
        <oboInOwl:hasOBONamespace>GAZ</oboInOwl:hasOBONamespace>
        <oboInOwl:id>GAZ:00372094</oboInOwl:id>
        <rdfs:label>Golubic Hydroelectric Power Plant</rdfs:label>
    </owl:NamedIndividual>
    


    <!-- http://purl.obolibrary.org/obo/GAZ_00372095 -->

    <owl:NamedIndividual rdf:about="http://purl.obolibrary.org/obo/GAZ_00372095">
        <obo:IAO_0000115>A hydroelectric power plant. Located under the Topolje waterfall in the Kovacici village, approximately 4.5 km northeast from Knin.</obo:IAO_0000115>
        <oboInOwl:hasOBONamespace>GAZ</oboInOwl:hasOBONamespace>
        <oboInOwl:id>GAZ:00372095</oboInOwl:id>
        <rdfs:label>Small Krcic Hydroelectric Power Plant</rdfs:label>
    </owl:NamedIndividual>
    


    <!-- http://purl.obolibrary.org/obo/GAZ_00372096 -->

    <owl:NamedIndividual rdf:about="http://purl.obolibrary.org/obo/GAZ_00372096">
        <obo:IAO_0000115>A hydroelectric power plant. Located 15 km downstream from the town of Knin. Constructed 1915.</obo:IAO_0000115>
        <oboInOwl:hasOBONamespace>GAZ</oboInOwl:hasOBONamespace>
        <oboInOwl:id>GAZ:00372096</oboInOwl:id>
        <rdfs:label>Miljacka Hydroelectric Power Plant</rdfs:label>
    </owl:NamedIndividual>
    


    <!-- http://purl.obolibrary.org/obo/GAZ_00372097 -->

    <owl:NamedIndividual rdf:about="http://purl.obolibrary.org/obo/GAZ_00372097">
        <obo:IAO_0000115>A hydroelectric power plant. Located near Miljevci. Constructed 1910.</obo:IAO_0000115>
        <oboInOwl:hasOBONamespace>GAZ</oboInOwl:hasOBONamespace>
        <oboInOwl:id>GAZ:00372097</oboInOwl:id>
        <rdfs:label>Roski Slap Hydroelectric Power Plant</rdfs:label>
    </owl:NamedIndividual>
    


    <!-- http://purl.obolibrary.org/obo/GAZ_00372099 -->

    <owl:NamedIndividual rdf:about="http://purl.obolibrary.org/obo/GAZ_00372099">
        <obo:IAO_0000115>Waterfalls and lakes.</obo:IAO_0000115>
        <oboInOwl:hasOBONamespace>GAZ</oboInOwl:hasOBONamespace>
        <oboInOwl:id>GAZ:00372099</oboInOwl:id>
        <rdfs:label>Skradinski buk</rdfs:label>
    </owl:NamedIndividual>
    


    <!-- http://purl.obolibrary.org/obo/GAZ_00372100 -->

    <owl:NamedIndividual rdf:about="http://purl.obolibrary.org/obo/GAZ_00372100">
        <obo:RO_0001025 rdf:resource="http://purl.obolibrary.org/obo/GAZ_00372099"/>
        <obo:IAO_0000115>An island.</obo:IAO_0000115>
        <oboInOwl:hasOBONamespace>GAZ</oboInOwl:hasOBONamespace>
        <oboInOwl:id>GAZ:00372100</oboInOwl:id>
        <rdfs:label>Visovac Island</rdfs:label>
    </owl:NamedIndividual>
    


    <!-- http://purl.obolibrary.org/obo/GAZ_00372204 -->

    <owl:NamedIndividual rdf:about="http://purl.obolibrary.org/obo/GAZ_00372204">
        <obo:IAO_0000115>A reservoir.</obo:IAO_0000115>
        <oboInOwl:hasOBONamespace>GAZ</oboInOwl:hasOBONamespace>
        <oboInOwl:id>GAZ:00372204</oboInOwl:id>
        <rdfs:label>Lake Varazdin</rdfs:label>
    </owl:NamedIndividual>
    


    <!-- http://purl.obolibrary.org/obo/GAZ_00372205 -->

    <owl:NamedIndividual rdf:about="http://purl.obolibrary.org/obo/GAZ_00372205">
        <obo:IAO_0000115>A reservoir.</obo:IAO_0000115>
        <oboInOwl:hasOBONamespace>GAZ</oboInOwl:hasOBONamespace>
        <oboInOwl:id>GAZ:00372205</oboInOwl:id>
        <rdfs:label>Lake Dubrava</rdfs:label>
    </owl:NamedIndividual>
    


    <!-- http://purl.obolibrary.org/obo/GAZ_00372215 -->

    <owl:NamedIndividual rdf:about="http://purl.obolibrary.org/obo/GAZ_00372215">
        <obo:IAO_0000115>A hydroelectric power plant.</obo:IAO_0000115>
        <oboInOwl:hasOBONamespace>GAZ</oboInOwl:hasOBONamespace>
        <oboInOwl:id>GAZ:00372215</oboInOwl:id>
        <rdfs:label>Cakovec Hydroelectric Power Plant</rdfs:label>
    </owl:NamedIndividual>
    


    <!-- http://purl.obolibrary.org/obo/GAZ_00372355 -->

    <owl:NamedIndividual rdf:about="http://purl.obolibrary.org/obo/GAZ_00372355">
        <obo:IAO_0000115>A reservoir; impounded by Cakovex Hydroelectric Power Plant.</obo:IAO_0000115>
        <oboInOwl:hasOBONamespace>GAZ</oboInOwl:hasOBONamespace>
        <oboInOwl:id>GAZ:00372355</oboInOwl:id>
        <rdfs:label>Varazdinsko jezero</rdfs:label>
    </owl:NamedIndividual>
    


    <!-- http://purl.obolibrary.org/obo/GAZ_00378648 -->

    <owl:NamedIndividual rdf:about="http://purl.obolibrary.org/obo/GAZ_00378648">
        <obo:IAO_0000115>A lake.</obo:IAO_0000115>
        <oboInOwl:hasOBONamespace>GAZ</oboInOwl:hasOBONamespace>
        <oboInOwl:id>GAZ:00378648</oboInOwl:id>
        <rdfs:label>Gajseva Lake</rdfs:label>
    </owl:NamedIndividual>
    


    <!-- http://purl.obolibrary.org/obo/GAZ_00378663 -->

    <owl:NamedIndividual rdf:about="http://purl.obolibrary.org/obo/GAZ_00378663">
        <oboInOwl:hasOBONamespace>GAZ</oboInOwl:hasOBONamespace>
        <oboInOwl:id>GAZ:00378663</oboInOwl:id>
        <rdfs:label>Medvode Hydroelectric Power Plant</rdfs:label>
    </owl:NamedIndividual>
    


    <!-- http://purl.obolibrary.org/obo/GAZ_00378729 -->

    <owl:NamedIndividual rdf:about="http://purl.obolibrary.org/obo/GAZ_00378729">
        <obo:IAO_0000115>A man-made lake.</obo:IAO_0000115>
        <oboInOwl:hasOBONamespace>GAZ</oboInOwl:hasOBONamespace>
        <oboInOwl:id>GAZ:00378729</oboInOwl:id>
        <rdfs:label>Ptujsko jezero</rdfs:label>
    </owl:NamedIndividual>
    


    <!-- http://purl.obolibrary.org/obo/GAZ_00378780 -->

    <owl:NamedIndividual rdf:about="http://purl.obolibrary.org/obo/GAZ_00378780">
        <obo:IAO_0000115>An island.</obo:IAO_0000115>
        <oboInOwl:hasOBONamespace>GAZ</oboInOwl:hasOBONamespace>
        <oboInOwl:id>GAZ:00378780</oboInOwl:id>
        <rdfs:label>Otocec</rdfs:label>
    </owl:NamedIndividual>
    


    <!-- http://purl.obolibrary.org/obo/GAZ_00378869 -->

    <owl:NamedIndividual rdf:about="http://purl.obolibrary.org/obo/GAZ_00378869">
        <obo:IAO_0000115>A river.</obo:IAO_0000115>
        <oboInOwl:hasOBONamespace>GAZ</oboInOwl:hasOBONamespace>
        <oboInOwl:id>GAZ:00378869</oboInOwl:id>
        <rdfs:label>Rusenski Lom</rdfs:label>
    </owl:NamedIndividual>
    


    <!-- http://purl.obolibrary.org/obo/GAZ_00378934 -->

    <owl:NamedIndividual rdf:about="http://purl.obolibrary.org/obo/GAZ_00378934">
        <obo:IAO_0000115>A dam.</obo:IAO_0000115>
        <oboInOwl:hasOBONamespace>GAZ</oboInOwl:hasOBONamespace>
        <oboInOwl:id>GAZ:00378934</oboInOwl:id>
        <rdfs:label>Aleksandar Stamboliyski Dam</rdfs:label>
    </owl:NamedIndividual>
    


    <!-- http://purl.obolibrary.org/obo/GAZ_00381635 -->

    <owl:NamedIndividual rdf:about="http://purl.obolibrary.org/obo/GAZ_00381635">
        <obo:IAO_0000115>A man-made lake.</obo:IAO_0000115>
        <oboInOwl:hasOBONamespace>GAZ</oboInOwl:hasOBONamespace>
        <oboInOwl:id>GAZ:00381635</oboInOwl:id>
        <rdfs:label>Lake Moarta</rdfs:label>
    </owl:NamedIndividual>
    


    <!-- http://purl.obolibrary.org/obo/GAZ_00381636 -->

    <owl:NamedIndividual rdf:about="http://purl.obolibrary.org/obo/GAZ_00381636">
        <obo:IAO_0000115>A man-made lake.</obo:IAO_0000115>
        <oboInOwl:hasOBONamespace>GAZ</oboInOwl:hasOBONamespace>
        <oboInOwl:id>GAZ:00381636</oboInOwl:id>
        <rdfs:label>Lake Ciocanesti I</rdfs:label>
    </owl:NamedIndividual>
    


    <!-- http://purl.obolibrary.org/obo/GAZ_00381637 -->

    <owl:NamedIndividual rdf:about="http://purl.obolibrary.org/obo/GAZ_00381637">
        <obo:IAO_0000115>A man-made lake.</obo:IAO_0000115>
        <oboInOwl:hasOBONamespace>GAZ</oboInOwl:hasOBONamespace>
        <oboInOwl:id>GAZ:00381637</oboInOwl:id>
        <rdfs:label>Lake Ciocanesti I</rdfs:label>
    </owl:NamedIndividual>
    


    <!-- http://purl.obolibrary.org/obo/GAZ_00381638 -->

    <owl:NamedIndividual rdf:about="http://purl.obolibrary.org/obo/GAZ_00381638">
        <obo:IAO_0000115>A man-made lake.</obo:IAO_0000115>
        <oboInOwl:hasOBONamespace>GAZ</oboInOwl:hasOBONamespace>
        <oboInOwl:id>GAZ:00381638</oboInOwl:id>
        <rdfs:label>Lake Crevedia VI</rdfs:label>
    </owl:NamedIndividual>
    


    <!-- http://purl.obolibrary.org/obo/GAZ_00381639 -->

    <owl:NamedIndividual rdf:about="http://purl.obolibrary.org/obo/GAZ_00381639">
        <obo:IAO_0000115>A man-made lake.</obo:IAO_0000115>
        <oboInOwl:hasOBONamespace>GAZ</oboInOwl:hasOBONamespace>
        <oboInOwl:id>GAZ:00381639</oboInOwl:id>
        <rdfs:label>Lake Buftea</rdfs:label>
    </owl:NamedIndividual>
    


    <!-- http://purl.obolibrary.org/obo/GAZ_00381640 -->

    <owl:NamedIndividual rdf:about="http://purl.obolibrary.org/obo/GAZ_00381640">
        <obo:IAO_0000115>A man-made lake.</obo:IAO_0000115>
        <oboInOwl:hasOBONamespace>GAZ</oboInOwl:hasOBONamespace>
        <oboInOwl:id>GAZ:00381640</oboInOwl:id>
        <rdfs:label>Lake Mogosoaia</rdfs:label>
    </owl:NamedIndividual>
    


    <!-- http://purl.obolibrary.org/obo/GAZ_00381641 -->

    <owl:NamedIndividual rdf:about="http://purl.obolibrary.org/obo/GAZ_00381641">
        <obo:IAO_0000115>A man-made lake.</obo:IAO_0000115>
        <oboInOwl:hasOBONamespace>GAZ</oboInOwl:hasOBONamespace>
        <oboInOwl:id>GAZ:00381641</oboInOwl:id>
        <rdfs:label>Lacul Chitila</rdfs:label>
    </owl:NamedIndividual>
    


    <!-- http://purl.obolibrary.org/obo/GAZ_00381642 -->

    <owl:NamedIndividual rdf:about="http://purl.obolibrary.org/obo/GAZ_00381642">
        <obo:IAO_0000115>A man-made lake.</obo:IAO_0000115>
        <oboInOwl:hasOBONamespace>GAZ</oboInOwl:hasOBONamespace>
        <oboInOwl:id>GAZ:00381642</oboInOwl:id>
        <rdfs:label>Lacul Straulesti</rdfs:label>
    </owl:NamedIndividual>
    


    <!-- http://purl.obolibrary.org/obo/GAZ_00381643 -->

    <owl:NamedIndividual rdf:about="http://purl.obolibrary.org/obo/GAZ_00381643">
        <obo:IAO_0000115>A man-made lake.</obo:IAO_0000115>
        <oboInOwl:hasOBONamespace>GAZ</oboInOwl:hasOBONamespace>
        <oboInOwl:id>GAZ:00381643</oboInOwl:id>
        <rdfs:label>Lacul Grivita</rdfs:label>
    </owl:NamedIndividual>
    


    <!-- http://purl.obolibrary.org/obo/GAZ_00381645 -->

    <owl:NamedIndividual rdf:about="http://purl.obolibrary.org/obo/GAZ_00381645">
        <obo:IAO_0000115>A man-made lake.</obo:IAO_0000115>
        <oboInOwl:hasOBONamespace>GAZ</oboInOwl:hasOBONamespace>
        <oboInOwl:id>GAZ:00381645</oboInOwl:id>
        <rdfs:label>Lacul Herastrau</rdfs:label>
    </owl:NamedIndividual>
    


    <!-- http://purl.obolibrary.org/obo/GAZ_00381646 -->

    <owl:NamedIndividual rdf:about="http://purl.obolibrary.org/obo/GAZ_00381646">
        <obo:IAO_0000115>A man-made lake.</obo:IAO_0000115>
        <oboInOwl:hasOBONamespace>GAZ</oboInOwl:hasOBONamespace>
        <oboInOwl:id>GAZ:00381646</oboInOwl:id>
        <rdfs:label>Lacul Floreasca</rdfs:label>
    </owl:NamedIndividual>
    


    <!-- http://purl.obolibrary.org/obo/GAZ_00381647 -->

    <owl:NamedIndividual rdf:about="http://purl.obolibrary.org/obo/GAZ_00381647">
        <obo:IAO_0000115>A man-made lake.</obo:IAO_0000115>
        <oboInOwl:hasOBONamespace>GAZ</oboInOwl:hasOBONamespace>
        <oboInOwl:id>GAZ:00381647</oboInOwl:id>
        <rdfs:label>Lacul Tei</rdfs:label>
    </owl:NamedIndividual>
    


    <!-- http://purl.obolibrary.org/obo/GAZ_00381649 -->

    <owl:NamedIndividual rdf:about="http://purl.obolibrary.org/obo/GAZ_00381649">
        <obo:IAO_0000115>A reservoir.</obo:IAO_0000115>
        <oboInOwl:hasOBONamespace>GAZ</oboInOwl:hasOBONamespace>
        <oboInOwl:id>GAZ:00381649</oboInOwl:id>
        <rdfs:label>Lacul Aroneanu</rdfs:label>
    </owl:NamedIndividual>
    


    <!-- http://purl.obolibrary.org/obo/GAZ_00381650 -->

    <owl:NamedIndividual rdf:about="http://purl.obolibrary.org/obo/GAZ_00381650">
        <obo:IAO_0000115>A reservoir.</obo:IAO_0000115>
        <oboInOwl:hasOBONamespace>GAZ</oboInOwl:hasOBONamespace>
        <oboInOwl:id>GAZ:00381650</oboInOwl:id>
        <rdfs:label>Lacul Dorobant</rdfs:label>
    </owl:NamedIndividual>
    


    <!-- http://purl.obolibrary.org/obo/GAZ_00381651 -->

    <owl:NamedIndividual rdf:about="http://purl.obolibrary.org/obo/GAZ_00381651">
        <obo:IAO_0000115>A man-made lake.</obo:IAO_0000115>
        <oboInOwl:hasOBONamespace>GAZ</oboInOwl:hasOBONamespace>
        <oboInOwl:id>GAZ:00381651</oboInOwl:id>
        <rdfs:label>Lacul Pantelimon</rdfs:label>
    </owl:NamedIndividual>
    


    <!-- http://purl.obolibrary.org/obo/GAZ_00381652 -->

    <owl:NamedIndividual rdf:about="http://purl.obolibrary.org/obo/GAZ_00381652">
        <obo:IAO_0000115>A man-made lake.</obo:IAO_0000115>
        <oboInOwl:hasOBONamespace>GAZ</oboInOwl:hasOBONamespace>
        <oboInOwl:id>GAZ:00381652</oboInOwl:id>
        <rdfs:label>Lacul Cernica</rdfs:label>
    </owl:NamedIndividual>
    


    <!-- http://purl.obolibrary.org/obo/GAZ_00381659 -->

    <owl:NamedIndividual rdf:about="http://purl.obolibrary.org/obo/GAZ_00381659">
        <obo:IAO_0000115>A man-made lake.</obo:IAO_0000115>
        <oboInOwl:hasOBONamespace>GAZ</oboInOwl:hasOBONamespace>
        <oboInOwl:id>GAZ:00381659</oboInOwl:id>
        <rdfs:label>Lacul Cismigiu</rdfs:label>
    </owl:NamedIndividual>
    


    <!-- http://purl.obolibrary.org/obo/GAZ_00381660 -->

    <owl:NamedIndividual rdf:about="http://purl.obolibrary.org/obo/GAZ_00381660">
        <obo:IAO_0000115>A man-made lake.</obo:IAO_0000115>
        <oboInOwl:hasOBONamespace>GAZ</oboInOwl:hasOBONamespace>
        <oboInOwl:id>GAZ:00381660</oboInOwl:id>
        <rdfs:label>Lacul Dambovita</rdfs:label>
    </owl:NamedIndividual>
    


    <!-- http://purl.obolibrary.org/obo/GAZ_00381662 -->

    <owl:NamedIndividual rdf:about="http://purl.obolibrary.org/obo/GAZ_00381662">
        <obo:IAO_0000115>A man-made lake.</obo:IAO_0000115>
        <oboInOwl:hasOBONamespace>GAZ</oboInOwl:hasOBONamespace>
        <oboInOwl:id>GAZ:00381662</oboInOwl:id>
        <rdfs:label>Lacul Vacaresti</rdfs:label>
    </owl:NamedIndividual>
    


    <!-- http://purl.obolibrary.org/obo/GAZ_00381663 -->

    <owl:NamedIndividual rdf:about="http://purl.obolibrary.org/obo/GAZ_00381663">
        <obo:IAO_0000115>A reservoir. Located 5 km from Pitesti.</obo:IAO_0000115>
        <oboInOwl:hasOBONamespace>GAZ</oboInOwl:hasOBONamespace>
        <oboInOwl:id>GAZ:00381663</oboInOwl:id>
        <rdfs:label>Barajul Budeasa</rdfs:label>
    </owl:NamedIndividual>
    


    <!-- http://purl.obolibrary.org/obo/GAZ_00381664 -->

    <owl:NamedIndividual rdf:about="http://purl.obolibrary.org/obo/GAZ_00381664">
        <obo:IAO_0000115>A man-made lake.</obo:IAO_0000115>
        <oboInOwl:hasOBONamespace>GAZ</oboInOwl:hasOBONamespace>
        <oboInOwl:id>GAZ:00381664</oboInOwl:id>
        <rdfs:label>Lacul Tineretului</rdfs:label>
    </owl:NamedIndividual>
    


    <!-- http://purl.obolibrary.org/obo/GAZ_00381671 -->

    <owl:NamedIndividual rdf:about="http://purl.obolibrary.org/obo/GAZ_00381671">
        <obo:IAO_0000115>A man-made lake.</obo:IAO_0000115>
        <oboInOwl:hasOBONamespace>GAZ</oboInOwl:hasOBONamespace>
        <oboInOwl:id>GAZ:00381671</oboInOwl:id>
        <rdfs:label>Lacul Baneasa</rdfs:label>
    </owl:NamedIndividual>
    


    <!-- http://purl.obolibrary.org/obo/GAZ_00381691 -->

    <owl:NamedIndividual rdf:about="http://purl.obolibrary.org/obo/GAZ_00381691">
        <obo:IAO_0000115>A reservoir.</obo:IAO_0000115>
        <oboInOwl:hasOBONamespace>GAZ</oboInOwl:hasOBONamespace>
        <oboInOwl:id>GAZ:00381691</oboInOwl:id>
        <rdfs:label>Lacul Chirita</rdfs:label>
    </owl:NamedIndividual>
    


    <!-- http://purl.obolibrary.org/obo/GAZ_00381695 -->

    <owl:NamedIndividual rdf:about="http://purl.obolibrary.org/obo/GAZ_00381695">
        <obo:IAO_0000115>A lake.</obo:IAO_0000115>
        <oboInOwl:hasOBONamespace>GAZ</oboInOwl:hasOBONamespace>
        <oboInOwl:id>GAZ:00381695</oboInOwl:id>
        <rdfs:label>Lacul Fundeni</rdfs:label>
    </owl:NamedIndividual>
    


    <!-- http://purl.obolibrary.org/obo/GAZ_00381696 -->

    <owl:NamedIndividual rdf:about="http://purl.obolibrary.org/obo/GAZ_00381696">
        <obo:IAO_0000115>A lake.</obo:IAO_0000115>
        <oboInOwl:hasOBONamespace>GAZ</oboInOwl:hasOBONamespace>
        <oboInOwl:id>GAZ:00381696</oboInOwl:id>
        <rdfs:label>Lacul Plumbuita</rdfs:label>
    </owl:NamedIndividual>
    


    <!-- http://purl.obolibrary.org/obo/GAZ_00381880 -->

    <owl:NamedIndividual rdf:about="http://purl.obolibrary.org/obo/GAZ_00381880">
        <obo:RO_0001025 rdf:resource="http://purl.obolibrary.org/obo/GAZ_00062020"/>
        <obo:IAO_0000115>An ice cave.</obo:IAO_0000115>
        <oboInOwl:hasOBONamespace>GAZ</oboInOwl:hasOBONamespace>
        <oboInOwl:id>GAZ:00381880</oboInOwl:id>
        <rdfs:label>Pestera Scarisoara</rdfs:label>
    </owl:NamedIndividual>
    


    <!-- http://purl.obolibrary.org/obo/GAZ_00382077 -->

    <owl:NamedIndividual rdf:about="http://purl.obolibrary.org/obo/GAZ_00382077">
        <obo:IAO_0000115>A reservoir.</obo:IAO_0000115>
        <oboInOwl:hasOBONamespace>GAZ</oboInOwl:hasOBONamespace>
        <oboInOwl:id>GAZ:00382077</oboInOwl:id>
        <rdfs:label>Barajul Frumoasa</rdfs:label>
    </owl:NamedIndividual>
    


    <!-- http://purl.obolibrary.org/obo/GAZ_00382078 -->

    <owl:NamedIndividual rdf:about="http://purl.obolibrary.org/obo/GAZ_00382078">
        <obo:IAO_0000115>A reservoir.</obo:IAO_0000115>
        <oboInOwl:hasOBONamespace>GAZ</oboInOwl:hasOBONamespace>
        <oboInOwl:id>GAZ:00382078</oboInOwl:id>
        <rdfs:label>Barajul Maneciu</rdfs:label>
    </owl:NamedIndividual>
    


    <!-- http://purl.obolibrary.org/obo/GAZ_00382079 -->

    <owl:NamedIndividual rdf:about="http://purl.obolibrary.org/obo/GAZ_00382079">
        <obo:IAO_0000115>A reservoir.</obo:IAO_0000115>
        <oboInOwl:hasOBONamespace>GAZ</oboInOwl:hasOBONamespace>
        <oboInOwl:id>GAZ:00382079</oboInOwl:id>
        <rdfs:label>Barajul Mesteacanul</rdfs:label>
    </owl:NamedIndividual>
    


    <!-- http://purl.obolibrary.org/obo/GAZ_00382080 -->

    <owl:NamedIndividual rdf:about="http://purl.obolibrary.org/obo/GAZ_00382080">
        <obo:IAO_0000115>A resrevoir.</obo:IAO_0000115>
        <oboInOwl:hasOBONamespace>GAZ</oboInOwl:hasOBONamespace>
        <oboInOwl:id>GAZ:00382080</oboInOwl:id>
        <rdfs:label>Barajul Motru</rdfs:label>
    </owl:NamedIndividual>
    


    <!-- http://purl.obolibrary.org/obo/GAZ_00382101 -->

    <owl:NamedIndividual rdf:about="http://purl.obolibrary.org/obo/GAZ_00382101">
        <obo:RO_0001025 rdf:resource="http://purl.obolibrary.org/obo/GAZ_00385671"/>
        <obo:IAO_0000115>A reservoir.</obo:IAO_0000115>
        <oboInOwl:hasOBONamespace>GAZ</oboInOwl:hasOBONamespace>
        <oboInOwl:id>GAZ:00382101</oboInOwl:id>
        <rdfs:label>Barajul Paltinu</rdfs:label>
    </owl:NamedIndividual>
    


    <!-- http://purl.obolibrary.org/obo/GAZ_00382102 -->

    <owl:NamedIndividual rdf:about="http://purl.obolibrary.org/obo/GAZ_00382102">
        <obo:IAO_0000115>A reservoir.</obo:IAO_0000115>
        <oboInOwl:hasOBONamespace>GAZ</oboInOwl:hasOBONamespace>
        <oboInOwl:id>GAZ:00382102</oboInOwl:id>
        <rdfs:label>Barajul Pecineagu</rdfs:label>
    </owl:NamedIndividual>
    


    <!-- http://purl.obolibrary.org/obo/GAZ_00382364 -->

    <owl:NamedIndividual rdf:about="http://purl.obolibrary.org/obo/GAZ_00382364">
        <oboInOwl:hasOBONamespace>GAZ</oboInOwl:hasOBONamespace>
        <oboInOwl:id>GAZ:00382364</oboInOwl:id>
        <rdfs:label>Moldova</rdfs:label>
    </owl:NamedIndividual>
    


    <!-- http://purl.obolibrary.org/obo/GAZ_00382526 -->

    <owl:NamedIndividual rdf:about="http://purl.obolibrary.org/obo/GAZ_00382526">
        <obo:IAO_0000115>A former dam. Failed 1991.</obo:IAO_0000115>
        <oboInOwl:hasOBONamespace>GAZ</oboInOwl:hasOBONamespace>
        <oboInOwl:id>GAZ:00382526</oboInOwl:id>
        <rdfs:label>Belci Dam</rdfs:label>
    </owl:NamedIndividual>
    


    <!-- http://purl.obolibrary.org/obo/GAZ_00382663 -->

    <owl:NamedIndividual rdf:about="http://purl.obolibrary.org/obo/GAZ_00382663">
        <obo:IAO_0000115>A river.</obo:IAO_0000115>
        <oboInOwl:hasOBONamespace>GAZ</oboInOwl:hasOBONamespace>
        <oboInOwl:id>GAZ:00382663</oboInOwl:id>
        <rdfs:label>Valea Neagra</rdfs:label>
    </owl:NamedIndividual>
    


    <!-- http://purl.obolibrary.org/obo/GAZ_00382664 -->

    <owl:NamedIndividual rdf:about="http://purl.obolibrary.org/obo/GAZ_00382664">
        <obo:IAO_0000115>A river.</obo:IAO_0000115>
        <oboInOwl:hasOBONamespace>GAZ</oboInOwl:hasOBONamespace>
        <oboInOwl:id>GAZ:00382664</oboInOwl:id>
        <rdfs:label>Orascu</rdfs:label>
    </owl:NamedIndividual>
    


    <!-- http://purl.obolibrary.org/obo/GAZ_00382665 -->

    <owl:NamedIndividual rdf:about="http://purl.obolibrary.org/obo/GAZ_00382665">
        <obo:IAO_0000115>A river.</obo:IAO_0000115>
        <oboInOwl:hasOBONamespace>GAZ</oboInOwl:hasOBONamespace>
        <oboInOwl:id>GAZ:00382665</oboInOwl:id>
        <rdfs:label>Valea Nesecata</rdfs:label>
    </owl:NamedIndividual>
    


    <!-- http://purl.obolibrary.org/obo/GAZ_00382666 -->

    <owl:NamedIndividual rdf:about="http://purl.obolibrary.org/obo/GAZ_00382666">
        <obo:IAO_0000115>A river.</obo:IAO_0000115>
        <oboInOwl:hasOBONamespace>GAZ</oboInOwl:hasOBONamespace>
        <oboInOwl:id>GAZ:00382666</oboInOwl:id>
        <rdfs:label>Bicaci</rdfs:label>
    </owl:NamedIndividual>
    


    <!-- http://purl.obolibrary.org/obo/GAZ_00382667 -->

    <owl:NamedIndividual rdf:about="http://purl.obolibrary.org/obo/GAZ_00382667">
        <obo:IAO_0000115>A river.</obo:IAO_0000115>
        <oboInOwl:hasOBONamespace>GAZ</oboInOwl:hasOBONamespace>
        <oboInOwl:id>GAZ:00382667</oboInOwl:id>
        <rdfs:label>Varies</rdfs:label>
    </owl:NamedIndividual>
    


    <!-- http://purl.obolibrary.org/obo/GAZ_00382671 -->

    <owl:NamedIndividual rdf:about="http://purl.obolibrary.org/obo/GAZ_00382671">
        <obo:RO_0001025 rdf:resource="http://purl.obolibrary.org/obo/GAZ_00382666"/>
        <obo:IAO_0000115>A lake. Located upstream of the village of Miersig.</obo:IAO_0000115>
        <oboInOwl:hasOBONamespace>GAZ</oboInOwl:hasOBONamespace>
        <oboInOwl:id>GAZ:00382671</oboInOwl:id>
        <rdfs:label>Lake Miersig</rdfs:label>
    </owl:NamedIndividual>
    


    <!-- http://purl.obolibrary.org/obo/GAZ_00383003 -->

    <owl:NamedIndividual rdf:about="http://purl.obolibrary.org/obo/GAZ_00383003">
        <obo:RO_0001025 rdf:resource="http://purl.obolibrary.org/obo/GAZ_00042216"/>
        <oboInOwl:hasOBONamespace>GAZ</oboInOwl:hasOBONamespace>
        <oboInOwl:id>GAZ:00383003</oboInOwl:id>
        <rdfs:label>Commune of Frecatei</rdfs:label>
    </owl:NamedIndividual>
    


    <!-- http://purl.obolibrary.org/obo/GAZ_00383009 -->

    <owl:NamedIndividual rdf:about="http://purl.obolibrary.org/obo/GAZ_00383009">
        <obo:RO_0001025 rdf:resource="http://purl.obolibrary.org/obo/GAZ_00042216"/>
        <oboInOwl:hasOBONamespace>GAZ</oboInOwl:hasOBONamespace>
        <oboInOwl:id>GAZ:00383009</oboInOwl:id>
        <rdfs:label>Commune of Marasu</rdfs:label>
    </owl:NamedIndividual>
    


    <!-- http://purl.obolibrary.org/obo/GAZ_00383340 -->

    <owl:NamedIndividual rdf:about="http://purl.obolibrary.org/obo/GAZ_00383340">
        <obo:IAO_0000115>A river.</obo:IAO_0000115>
        <oboInOwl:hasOBONamespace>GAZ</oboInOwl:hasOBONamespace>
        <oboInOwl:id>GAZ:00383340</oboInOwl:id>
        <rdfs:label>Oltet [Brasov]</rdfs:label>
    </owl:NamedIndividual>
    


    <!-- http://purl.obolibrary.org/obo/GAZ_00383545 -->

    <owl:NamedIndividual rdf:about="http://purl.obolibrary.org/obo/GAZ_00383545">
        <obo:IAO_0000115>An island. A protected area.</obo:IAO_0000115>
        <oboInOwl:hasOBONamespace>GAZ</oboInOwl:hasOBONamespace>
        <oboInOwl:id>GAZ:00383545</oboInOwl:id>
        <rdfs:label>Ostrovul Ciocanesti</rdfs:label>
    </owl:NamedIndividual>
    


    <!-- http://purl.obolibrary.org/obo/GAZ_00383550 -->

    <owl:NamedIndividual rdf:about="http://purl.obolibrary.org/obo/GAZ_00383550">
        <obo:IAO_0000115>A man-made lake.</obo:IAO_0000115>
        <oboInOwl:hasOBONamespace>GAZ</oboInOwl:hasOBONamespace>
        <oboInOwl:id>GAZ:00383550</oboInOwl:id>
        <rdfs:label>Tierna</rdfs:label>
    </owl:NamedIndividual>
    


    <!-- http://purl.obolibrary.org/obo/GAZ_00383921 -->

    <owl:NamedIndividual rdf:about="http://purl.obolibrary.org/obo/GAZ_00383921">
        <obo:IAO_0000115>A reservoir.</obo:IAO_0000115>
        <oboInOwl:hasOBONamespace>GAZ</oboInOwl:hasOBONamespace>
        <oboInOwl:id>GAZ:00383921</oboInOwl:id>
        <rdfs:label>Barajul Poiana Uzului</rdfs:label>
    </owl:NamedIndividual>
    


    <!-- http://purl.obolibrary.org/obo/GAZ_00383923 -->

    <owl:NamedIndividual rdf:about="http://purl.obolibrary.org/obo/GAZ_00383923">
        <obo:IAO_0000115>A lake.</obo:IAO_0000115>
        <oboInOwl:hasOBONamespace>GAZ</oboInOwl:hasOBONamespace>
        <oboInOwl:id>GAZ:00383923</oboInOwl:id>
        <rdfs:label>Lake Scropoasa</rdfs:label>
    </owl:NamedIndividual>
    


    <!-- http://purl.obolibrary.org/obo/GAZ_00383940 -->

    <owl:NamedIndividual rdf:about="http://purl.obolibrary.org/obo/GAZ_00383940">
        <oboInOwl:hasOBONamespace>GAZ</oboInOwl:hasOBONamespace>
        <oboInOwl:id>GAZ:00383940</oboInOwl:id>
        <rdfs:label>Slanic de Gura Ocnitei</rdfs:label>
    </owl:NamedIndividual>
    


    <!-- http://purl.obolibrary.org/obo/GAZ_00383941 -->

    <owl:NamedIndividual rdf:about="http://purl.obolibrary.org/obo/GAZ_00383941">
        <oboInOwl:hasOBONamespace>GAZ</oboInOwl:hasOBONamespace>
        <oboInOwl:id>GAZ:00383941</oboInOwl:id>
        <rdfs:label>Pascov</rdfs:label>
    </owl:NamedIndividual>
    


    <!-- http://purl.obolibrary.org/obo/GAZ_00383942 -->

    <owl:NamedIndividual rdf:about="http://purl.obolibrary.org/obo/GAZ_00383942">
        <oboInOwl:hasOBONamespace>GAZ</oboInOwl:hasOBONamespace>
        <oboInOwl:id>GAZ:00383942</oboInOwl:id>
        <rdfs:label>Crivat</rdfs:label>
    </owl:NamedIndividual>
    


    <!-- http://purl.obolibrary.org/obo/GAZ_00383943 -->

    <owl:NamedIndividual rdf:about="http://purl.obolibrary.org/obo/GAZ_00383943">
        <oboInOwl:hasOBONamespace>GAZ</oboInOwl:hasOBONamespace>
        <oboInOwl:id>GAZ:00383943</oboInOwl:id>
        <rdfs:label>Cricovul Dulce</rdfs:label>
    </owl:NamedIndividual>
    


    <!-- http://purl.obolibrary.org/obo/GAZ_00383944 -->

    <owl:NamedIndividual rdf:about="http://purl.obolibrary.org/obo/GAZ_00383944">
        <obo:IAO_0000115>A river.</obo:IAO_0000115>
        <oboInOwl:hasOBONamespace>GAZ</oboInOwl:hasOBONamespace>
        <oboInOwl:id>GAZ:00383944</oboInOwl:id>
        <rdfs:label>Prahova</rdfs:label>
    </owl:NamedIndividual>
    


    <!-- http://purl.obolibrary.org/obo/GAZ_00383945 -->

    <owl:NamedIndividual rdf:about="http://purl.obolibrary.org/obo/GAZ_00383945">
        <oboInOwl:hasOBONamespace>GAZ</oboInOwl:hasOBONamespace>
        <oboInOwl:id>GAZ:00383945</oboInOwl:id>
        <rdfs:label>Sarata</rdfs:label>
    </owl:NamedIndividual>
    


    <!-- http://purl.obolibrary.org/obo/GAZ_00383946 -->

    <owl:NamedIndividual rdf:about="http://purl.obolibrary.org/obo/GAZ_00383946">
        <oboInOwl:hasOBONamespace>GAZ</oboInOwl:hasOBONamespace>
        <oboInOwl:id>GAZ:00383946</oboInOwl:id>
        <rdfs:label>Cotorca</rdfs:label>
    </owl:NamedIndividual>
    


    <!-- http://purl.obolibrary.org/obo/GAZ_00383947 -->

    <owl:NamedIndividual rdf:about="http://purl.obolibrary.org/obo/GAZ_00383947">
        <oboInOwl:hasOBONamespace>GAZ</oboInOwl:hasOBONamespace>
        <oboInOwl:id>GAZ:00383947</oboInOwl:id>
        <rdfs:label>Saratuica</rdfs:label>
    </owl:NamedIndividual>
    


    <!-- http://purl.obolibrary.org/obo/GAZ_00383948 -->

    <owl:NamedIndividual rdf:about="http://purl.obolibrary.org/obo/GAZ_00383948">
        <oboInOwl:hasOBONamespace>GAZ</oboInOwl:hasOBONamespace>
        <oboInOwl:id>GAZ:00383948</oboInOwl:id>
        <rdfs:label>Strachina</rdfs:label>
    </owl:NamedIndividual>
    


    <!-- http://purl.obolibrary.org/obo/GAZ_00383949 -->

    <owl:NamedIndividual rdf:about="http://purl.obolibrary.org/obo/GAZ_00383949">
        <oboInOwl:hasOBONamespace>GAZ</oboInOwl:hasOBONamespace>
        <oboInOwl:id>GAZ:00383949</oboInOwl:id>
        <rdfs:label>Valea Doamnelor</rdfs:label>
    </owl:NamedIndividual>
    


    <!-- http://purl.obolibrary.org/obo/GAZ_00383950 -->

    <owl:NamedIndividual rdf:about="http://purl.obolibrary.org/obo/GAZ_00383950">
        <oboInOwl:hasOBONamespace>GAZ</oboInOwl:hasOBONamespace>
        <oboInOwl:id>GAZ:00383950</oboInOwl:id>
        <rdfs:label>Valea Suchenitei Horoaba</rdfs:label>
    </owl:NamedIndividual>
    


    <!-- http://purl.obolibrary.org/obo/GAZ_00383951 -->

    <owl:NamedIndividual rdf:about="http://purl.obolibrary.org/obo/GAZ_00383951">
        <oboInOwl:hasOBONamespace>GAZ</oboInOwl:hasOBONamespace>
        <oboInOwl:id>GAZ:00383951</oboInOwl:id>
        <rdfs:label>Coteanu</rdfs:label>
    </owl:NamedIndividual>
    


    <!-- http://purl.obolibrary.org/obo/GAZ_00383952 -->

    <owl:NamedIndividual rdf:about="http://purl.obolibrary.org/obo/GAZ_00383952">
        <oboInOwl:hasOBONamespace>GAZ</oboInOwl:hasOBONamespace>
        <oboInOwl:id>GAZ:00383952</oboInOwl:id>
        <rdfs:label>Valea Vacariei</rdfs:label>
    </owl:NamedIndividual>
    


    <!-- http://purl.obolibrary.org/obo/GAZ_00383953 -->

    <owl:NamedIndividual rdf:about="http://purl.obolibrary.org/obo/GAZ_00383953">
        <oboInOwl:hasOBONamespace>GAZ</oboInOwl:hasOBONamespace>
        <oboInOwl:id>GAZ:00383953</oboInOwl:id>
        <rdfs:label>Tataru</rdfs:label>
    </owl:NamedIndividual>
    


    <!-- http://purl.obolibrary.org/obo/GAZ_00383954 -->

    <owl:NamedIndividual rdf:about="http://purl.obolibrary.org/obo/GAZ_00383954">
        <oboInOwl:hasOBONamespace>GAZ</oboInOwl:hasOBONamespace>
        <oboInOwl:id>GAZ:00383954</oboInOwl:id>
        <rdfs:label>Galgoi</rdfs:label>
    </owl:NamedIndividual>
    


    <!-- http://purl.obolibrary.org/obo/GAZ_00383955 -->

    <owl:NamedIndividual rdf:about="http://purl.obolibrary.org/obo/GAZ_00383955">
        <oboInOwl:hasOBONamespace>GAZ</oboInOwl:hasOBONamespace>
        <oboInOwl:id>GAZ:00383955</oboInOwl:id>
        <rdfs:label>Mircea</rdfs:label>
    </owl:NamedIndividual>
    


    <!-- http://purl.obolibrary.org/obo/GAZ_00383956 -->

    <owl:NamedIndividual rdf:about="http://purl.obolibrary.org/obo/GAZ_00383956">
        <oboInOwl:hasOBONamespace>GAZ</oboInOwl:hasOBONamespace>
        <oboInOwl:id>GAZ:00383956</oboInOwl:id>
        <rdfs:label>Bolboci</rdfs:label>
    </owl:NamedIndividual>
    


    <!-- http://purl.obolibrary.org/obo/GAZ_00383957 -->

    <owl:NamedIndividual rdf:about="http://purl.obolibrary.org/obo/GAZ_00383957">
        <oboInOwl:hasOBONamespace>GAZ</oboInOwl:hasOBONamespace>
        <oboInOwl:id>GAZ:00383957</oboInOwl:id>
        <rdfs:label>Lucacila</rdfs:label>
    </owl:NamedIndividual>
    


    <!-- http://purl.obolibrary.org/obo/GAZ_00383958 -->

    <owl:NamedIndividual rdf:about="http://purl.obolibrary.org/obo/GAZ_00383958">
        <oboInOwl:hasOBONamespace>GAZ</oboInOwl:hasOBONamespace>
        <oboInOwl:id>GAZ:00383958</oboInOwl:id>
        <rdfs:label>Zanoaga</rdfs:label>
    </owl:NamedIndividual>
    


    <!-- http://purl.obolibrary.org/obo/GAZ_00383959 -->

    <owl:NamedIndividual rdf:about="http://purl.obolibrary.org/obo/GAZ_00383959">
        <oboInOwl:hasOBONamespace>GAZ</oboInOwl:hasOBONamespace>
        <oboInOwl:id>GAZ:00383959</oboInOwl:id>
        <rdfs:label>Valea Cabanierului</rdfs:label>
    </owl:NamedIndividual>
    


    <!-- http://purl.obolibrary.org/obo/GAZ_00383960 -->

    <owl:NamedIndividual rdf:about="http://purl.obolibrary.org/obo/GAZ_00383960">
        <oboInOwl:hasOBONamespace>GAZ</oboInOwl:hasOBONamespace>
        <oboInOwl:id>GAZ:00383960</oboInOwl:id>
        <rdfs:label>Bratei</rdfs:label>
    </owl:NamedIndividual>
    


    <!-- http://purl.obolibrary.org/obo/GAZ_00383961 -->

    <owl:NamedIndividual rdf:about="http://purl.obolibrary.org/obo/GAZ_00383961">
        <oboInOwl:hasOBONamespace>GAZ</oboInOwl:hasOBONamespace>
        <oboInOwl:id>GAZ:00383961</oboInOwl:id>
        <rdfs:label>Ratei</rdfs:label>
    </owl:NamedIndividual>
    


    <!-- http://purl.obolibrary.org/obo/GAZ_00383962 -->

    <owl:NamedIndividual rdf:about="http://purl.obolibrary.org/obo/GAZ_00383962">
        <oboInOwl:hasOBONamespace>GAZ</oboInOwl:hasOBONamespace>
        <oboInOwl:id>GAZ:00383962</oboInOwl:id>
        <rdfs:label>Raciu</rdfs:label>
    </owl:NamedIndividual>
    


    <!-- http://purl.obolibrary.org/obo/GAZ_00383963 -->

    <owl:NamedIndividual rdf:about="http://purl.obolibrary.org/obo/GAZ_00383963">
        <oboInOwl:hasOBONamespace>GAZ</oboInOwl:hasOBONamespace>
        <oboInOwl:id>GAZ:00383963</oboInOwl:id>
        <rdfs:label>Valea Doicii</rdfs:label>
    </owl:NamedIndividual>
    


    <!-- http://purl.obolibrary.org/obo/GAZ_00383964 -->

    <owl:NamedIndividual rdf:about="http://purl.obolibrary.org/obo/GAZ_00383964">
        <oboInOwl:hasOBONamespace>GAZ</oboInOwl:hasOBONamespace>
        <oboInOwl:id>GAZ:00383964</oboInOwl:id>
        <rdfs:label>Seciul cu Colti</rdfs:label>
    </owl:NamedIndividual>
    


    <!-- http://purl.obolibrary.org/obo/GAZ_00383965 -->

    <owl:NamedIndividual rdf:about="http://purl.obolibrary.org/obo/GAZ_00383965">
        <oboInOwl:hasOBONamespace>GAZ</oboInOwl:hasOBONamespace>
        <oboInOwl:id>GAZ:00383965</oboInOwl:id>
        <rdfs:label>Voivodeni</rdfs:label>
    </owl:NamedIndividual>
    


    <!-- http://purl.obolibrary.org/obo/GAZ_00383966 -->

    <owl:NamedIndividual rdf:about="http://purl.obolibrary.org/obo/GAZ_00383966">
        <oboInOwl:hasOBONamespace>GAZ</oboInOwl:hasOBONamespace>
        <oboInOwl:id>GAZ:00383966</oboInOwl:id>
        <rdfs:label>Tata</rdfs:label>
    </owl:NamedIndividual>
    


    <!-- http://purl.obolibrary.org/obo/GAZ_00383967 -->

    <owl:NamedIndividual rdf:about="http://purl.obolibrary.org/obo/GAZ_00383967">
        <oboInOwl:hasOBONamespace>GAZ</oboInOwl:hasOBONamespace>
        <oboInOwl:id>GAZ:00383967</oboInOwl:id>
        <rdfs:label>Ialomicioara</rdfs:label>
    </owl:NamedIndividual>
    


    <!-- http://purl.obolibrary.org/obo/GAZ_00383968 -->

    <owl:NamedIndividual rdf:about="http://purl.obolibrary.org/obo/GAZ_00383968">
        <oboInOwl:hasOBONamespace>GAZ</oboInOwl:hasOBONamespace>
        <oboInOwl:id>GAZ:00383968</oboInOwl:id>
        <rdfs:label>Vulcana</rdfs:label>
    </owl:NamedIndividual>
    


    <!-- http://purl.obolibrary.org/obo/GAZ_00383969 -->

    <owl:NamedIndividual rdf:about="http://purl.obolibrary.org/obo/GAZ_00383969">
        <oboInOwl:hasOBONamespace>GAZ</oboInOwl:hasOBONamespace>
        <oboInOwl:id>GAZ:00383969</oboInOwl:id>
        <rdfs:label>Glod</rdfs:label>
    </owl:NamedIndividual>
    


    <!-- http://purl.obolibrary.org/obo/GAZ_00383970 -->

    <owl:NamedIndividual rdf:about="http://purl.obolibrary.org/obo/GAZ_00383970">
        <oboInOwl:hasOBONamespace>GAZ</oboInOwl:hasOBONamespace>
        <oboInOwl:id>GAZ:00383970</oboInOwl:id>
        <rdfs:label>Ruda</rdfs:label>
    </owl:NamedIndividual>
    


    <!-- http://purl.obolibrary.org/obo/GAZ_00383971 -->

    <owl:NamedIndividual rdf:about="http://purl.obolibrary.org/obo/GAZ_00383971">
        <oboInOwl:hasOBONamespace>GAZ</oboInOwl:hasOBONamespace>
        <oboInOwl:id>GAZ:00383971</oboInOwl:id>
        <rdfs:label>Racovita</rdfs:label>
    </owl:NamedIndividual>
    


    <!-- http://purl.obolibrary.org/obo/GAZ_00383972 -->

    <owl:NamedIndividual rdf:about="http://purl.obolibrary.org/obo/GAZ_00383972">
        <oboInOwl:hasOBONamespace>GAZ</oboInOwl:hasOBONamespace>
        <oboInOwl:id>GAZ:00383972</oboInOwl:id>
        <rdfs:label>Snagov</rdfs:label>
    </owl:NamedIndividual>
    


    <!-- http://purl.obolibrary.org/obo/GAZ_00383973 -->

    <owl:NamedIndividual rdf:about="http://purl.obolibrary.org/obo/GAZ_00383973">
        <oboInOwl:hasOBONamespace>GAZ</oboInOwl:hasOBONamespace>
        <oboInOwl:id>GAZ:00383973</oboInOwl:id>
        <rdfs:label>Vlasia</rdfs:label>
    </owl:NamedIndividual>
    


    <!-- http://purl.obolibrary.org/obo/GAZ_00383974 -->

    <owl:NamedIndividual rdf:about="http://purl.obolibrary.org/obo/GAZ_00383974">
        <oboInOwl:hasOBONamespace>GAZ</oboInOwl:hasOBONamespace>
        <oboInOwl:id>GAZ:00383974</oboInOwl:id>
        <rdfs:label>Comana</rdfs:label>
    </owl:NamedIndividual>
    


    <!-- http://purl.obolibrary.org/obo/GAZ_00384414 -->

    <owl:NamedIndividual rdf:about="http://purl.obolibrary.org/obo/GAZ_00384414">
        <obo:IAO_0000115>A river.</obo:IAO_0000115>
        <oboInOwl:hasOBONamespace>GAZ</oboInOwl:hasOBONamespace>
        <oboInOwl:id>GAZ:00384414</oboInOwl:id>
        <rdfs:label>Valea Ciresului</rdfs:label>
    </owl:NamedIndividual>
    


    <!-- http://purl.obolibrary.org/obo/GAZ_00384415 -->

    <owl:NamedIndividual rdf:about="http://purl.obolibrary.org/obo/GAZ_00384415">
        <obo:IAO_0000115>A river.</obo:IAO_0000115>
        <oboInOwl:hasOBONamespace>GAZ</oboInOwl:hasOBONamespace>
        <oboInOwl:id>GAZ:00384415</oboInOwl:id>
        <rdfs:label>Leurda</rdfs:label>
    </owl:NamedIndividual>
    


    <!-- http://purl.obolibrary.org/obo/GAZ_00384416 -->

    <owl:NamedIndividual rdf:about="http://purl.obolibrary.org/obo/GAZ_00384416">
        <obo:IAO_0000115>A river.</obo:IAO_0000115>
        <oboInOwl:hasOBONamespace>GAZ</oboInOwl:hasOBONamespace>
        <oboInOwl:id>GAZ:00384416</oboInOwl:id>
        <rdfs:label>Rosiuta</rdfs:label>
    </owl:NamedIndividual>
    


    <!-- http://purl.obolibrary.org/obo/GAZ_00384417 -->

    <owl:NamedIndividual rdf:about="http://purl.obolibrary.org/obo/GAZ_00384417">
        <obo:IAO_0000115>A river.</obo:IAO_0000115>
        <oboInOwl:hasOBONamespace>GAZ</oboInOwl:hasOBONamespace>
        <oboInOwl:id>GAZ:00384417</oboInOwl:id>
        <rdfs:label>Stirbet</rdfs:label>
    </owl:NamedIndividual>
    


    <!-- http://purl.obolibrary.org/obo/GAZ_00384420 -->

    <owl:NamedIndividual rdf:about="http://purl.obolibrary.org/obo/GAZ_00384420">
        <obo:IAO_0000115>A river.</obo:IAO_0000115>
        <oboInOwl:hasOBONamespace>GAZ</oboInOwl:hasOBONamespace>
        <oboInOwl:id>GAZ:00384420</oboInOwl:id>
        <rdfs:label>Brebina</rdfs:label>
    </owl:NamedIndividual>
    


    <!-- http://purl.obolibrary.org/obo/GAZ_00384448 -->

    <owl:NamedIndividual rdf:about="http://purl.obolibrary.org/obo/GAZ_00384448">
        <obo:IAO_0000115>A river.</obo:IAO_0000115>
        <oboInOwl:hasOBONamespace>GAZ</oboInOwl:hasOBONamespace>
        <oboInOwl:id>GAZ:00384448</oboInOwl:id>
        <rdfs:label>Metei</rdfs:label>
    </owl:NamedIndividual>
    


    <!-- http://purl.obolibrary.org/obo/GAZ_00384449 -->

    <owl:NamedIndividual rdf:about="http://purl.obolibrary.org/obo/GAZ_00384449">
        <obo:IAO_0000115>A river.</obo:IAO_0000115>
        <oboInOwl:hasOBONamespace>GAZ</oboInOwl:hasOBONamespace>
        <oboInOwl:id>GAZ:00384449</oboInOwl:id>
        <rdfs:label>Paraul Pitiocariei</rdfs:label>
    </owl:NamedIndividual>
    


    <!-- http://purl.obolibrary.org/obo/GAZ_00384450 -->

    <owl:NamedIndividual rdf:about="http://purl.obolibrary.org/obo/GAZ_00384450">
        <obo:IAO_0000115>A river.</obo:IAO_0000115>
        <oboInOwl:hasOBONamespace>GAZ</oboInOwl:hasOBONamespace>
        <oboInOwl:id>GAZ:00384450</oboInOwl:id>
        <rdfs:label>Cupasul Mic</rdfs:label>
    </owl:NamedIndividual>
    


    <!-- http://purl.obolibrary.org/obo/GAZ_00384465 -->

    <owl:NamedIndividual rdf:about="http://purl.obolibrary.org/obo/GAZ_00384465">
        <obo:IAO_0000115>A river.</obo:IAO_0000115>
        <oboInOwl:hasOBONamespace>GAZ</oboInOwl:hasOBONamespace>
        <oboInOwl:id>GAZ:00384465</oboInOwl:id>
        <rdfs:label>Neagra Mare</rdfs:label>
    </owl:NamedIndividual>
    


    <!-- http://purl.obolibrary.org/obo/GAZ_00384466 -->

    <owl:NamedIndividual rdf:about="http://purl.obolibrary.org/obo/GAZ_00384466">
        <obo:IAO_0000115>A river.</obo:IAO_0000115>
        <oboInOwl:hasOBONamespace>GAZ</oboInOwl:hasOBONamespace>
        <oboInOwl:id>GAZ:00384466</oboInOwl:id>
        <rdfs:label>Neagra Mica</rdfs:label>
    </owl:NamedIndividual>
    


    <!-- http://purl.obolibrary.org/obo/GAZ_00384922 -->

    <owl:NamedIndividual rdf:about="http://purl.obolibrary.org/obo/GAZ_00384922">
        <obo:IAO_0000115>A river.</obo:IAO_0000115>
        <oboInOwl:hasOBONamespace>GAZ</oboInOwl:hasOBONamespace>
        <oboInOwl:id>GAZ:00384922</oboInOwl:id>
        <rdfs:label>Raul Agrij</rdfs:label>
    </owl:NamedIndividual>
    


    <!-- http://purl.obolibrary.org/obo/GAZ_00385318 -->

    <owl:NamedIndividual rdf:about="http://purl.obolibrary.org/obo/GAZ_00385318">
        <obo:RO_0001025 rdf:resource="http://purl.obolibrary.org/obo/GAZ_00061962"/>
        <obo:IAO_0000115>A protected area.</obo:IAO_0000115>
        <oboInOwl:hasOBONamespace>GAZ</oboInOwl:hasOBONamespace>
        <oboInOwl:id>GAZ:00385318</oboInOwl:id>
        <rdfs:label>Parcul National Ceahlau</rdfs:label>
    </owl:NamedIndividual>
    


    <!-- http://purl.obolibrary.org/obo/GAZ_00385476 -->

    <owl:NamedIndividual rdf:about="http://purl.obolibrary.org/obo/GAZ_00385476">
        <obo:RO_0001025 rdf:resource="http://purl.obolibrary.org/obo/GAZ_00061695"/>
        <obo:IAO_0000115>A park.</obo:IAO_0000115>
        <oboInOwl:hasOBONamespace>GAZ</oboInOwl:hasOBONamespace>
        <oboInOwl:id>GAZ:00385476</oboInOwl:id>
        <rdfs:label>Parcul Natural Vanatori-Neamt</rdfs:label>
    </owl:NamedIndividual>
    


    <!-- http://purl.obolibrary.org/obo/GAZ_00385671 -->

    <owl:NamedIndividual rdf:about="http://purl.obolibrary.org/obo/GAZ_00385671">
        <obo:IAO_0000115>A river.</obo:IAO_0000115>
        <oboInOwl:hasOBONamespace>GAZ</oboInOwl:hasOBONamespace>
        <oboInOwl:id>GAZ:00385671</oboInOwl:id>
        <rdfs:label>Doftana</rdfs:label>
    </owl:NamedIndividual>
    


    <!-- http://purl.obolibrary.org/obo/GAZ_00386424 -->

    <owl:NamedIndividual rdf:about="http://purl.obolibrary.org/obo/GAZ_00386424">
        <obo:IAO_0000115>An island. Located near Islaz.</obo:IAO_0000115>
        <oboInOwl:hasOBONamespace>GAZ</oboInOwl:hasOBONamespace>
        <oboInOwl:id>GAZ:00386424</oboInOwl:id>
        <rdfs:label>Ostrovul Mare</rdfs:label>
    </owl:NamedIndividual>
    


    <!-- http://purl.obolibrary.org/obo/GAZ_00386425 -->

    <owl:NamedIndividual rdf:about="http://purl.obolibrary.org/obo/GAZ_00386425">
        <obo:IAO_0000115>An island. Located near Islaz.</obo:IAO_0000115>
        <oboInOwl:hasOBONamespace>GAZ</oboInOwl:hasOBONamespace>
        <oboInOwl:id>GAZ:00386425</oboInOwl:id>
        <rdfs:label>Ostrovul Calnovat</rdfs:label>
    </owl:NamedIndividual>
    


    <!-- http://purl.obolibrary.org/obo/GAZ_00386426 -->

    <owl:NamedIndividual rdf:about="http://purl.obolibrary.org/obo/GAZ_00386426">
        <obo:RO_0001025 rdf:resource="http://purl.obolibrary.org/obo/GAZ_00386424"/>
        <obo:IAO_0000115>A protected area.</obo:IAO_0000115>
        <oboInOwl:hasOBONamespace>GAZ</oboInOwl:hasOBONamespace>
        <oboInOwl:id>GAZ:00386426</oboInOwl:id>
        <rdfs:label>Rezervatia naturala Ostrovul Mare</rdfs:label>
    </owl:NamedIndividual>
    


    <!-- http://purl.obolibrary.org/obo/GAZ_00386530 -->

    <owl:NamedIndividual rdf:about="http://purl.obolibrary.org/obo/GAZ_00386530">
        <obo:RO_0001025 rdf:resource="http://purl.obolibrary.org/obo/GAZ_00042218"/>
        <obo:IAO_0000115>An archeological site. Located at the mouth of the Danube Delta in Romania. Roman.</obo:IAO_0000115>
        <oboInOwl:hasOBONamespace>GAZ</oboInOwl:hasOBONamespace>
        <oboInOwl:id>GAZ:00386530</oboInOwl:id>
        <rdfs:label>Halmyris</rdfs:label>
    </owl:NamedIndividual>
    


    <!-- http://purl.obolibrary.org/obo/GAZ_00386581 -->

    <owl:NamedIndividual rdf:about="http://purl.obolibrary.org/obo/GAZ_00386581">
        <obo:RO_0001025 rdf:resource="http://purl.obolibrary.org/obo/GAZ_00042218"/>
        <obo:IAO_0000115>A lake.</obo:IAO_0000115>
        <oboInOwl:hasOBONamespace>GAZ</oboInOwl:hasOBONamespace>
        <oboInOwl:id>GAZ:00386581</oboInOwl:id>
        <rdfs:label>Lacul Babadag</rdfs:label>
    </owl:NamedIndividual>
    


    <!-- http://purl.obolibrary.org/obo/GAZ_00386592 -->

    <owl:NamedIndividual rdf:about="http://purl.obolibrary.org/obo/GAZ_00386592">
        <obo:RO_0001025 rdf:resource="http://purl.obolibrary.org/obo/GAZ_00042218"/>
        <obo:IAO_0000115>A lake.</obo:IAO_0000115>
        <oboInOwl:hasOBONamespace>GAZ</oboInOwl:hasOBONamespace>
        <oboInOwl:id>GAZ:00386592</oboInOwl:id>
        <rdfs:label>Lacul Rotund</rdfs:label>
    </owl:NamedIndividual>
    


    <!-- http://purl.obolibrary.org/obo/GAZ_00386593 -->

    <owl:NamedIndividual rdf:about="http://purl.obolibrary.org/obo/GAZ_00386593">
        <obo:RO_0001025 rdf:resource="http://purl.obolibrary.org/obo/GAZ_00042218"/>
        <obo:IAO_0000115>A lake.</obo:IAO_0000115>
        <oboInOwl:hasOBONamespace>GAZ</oboInOwl:hasOBONamespace>
        <oboInOwl:id>GAZ:00386593</oboInOwl:id>
        <rdfs:label>Lacul Saun</rdfs:label>
    </owl:NamedIndividual>
    


    <!-- http://purl.obolibrary.org/obo/GAZ_00386594 -->

    <owl:NamedIndividual rdf:about="http://purl.obolibrary.org/obo/GAZ_00386594">
        <obo:RO_0001025 rdf:resource="http://purl.obolibrary.org/obo/GAZ_00042218"/>
        <obo:IAO_0000115>A lake.</obo:IAO_0000115>
        <oboInOwl:hasOBONamespace>GAZ</oboInOwl:hasOBONamespace>
        <oboInOwl:id>GAZ:00386594</oboInOwl:id>
        <rdfs:label>Lacul Telincea</rdfs:label>
    </owl:NamedIndividual>
    


    <!-- http://purl.obolibrary.org/obo/GAZ_00386595 -->

    <owl:NamedIndividual rdf:about="http://purl.obolibrary.org/obo/GAZ_00386595">
        <obo:RO_0001025 rdf:resource="http://purl.obolibrary.org/obo/GAZ_00042218"/>
        <obo:IAO_0000115>A lake.</obo:IAO_0000115>
        <oboInOwl:hasOBONamespace>GAZ</oboInOwl:hasOBONamespace>
        <oboInOwl:id>GAZ:00386595</oboInOwl:id>
        <rdfs:label>Lacul Ghiolul Pietrei</rdfs:label>
    </owl:NamedIndividual>
    


    <!-- http://purl.obolibrary.org/obo/GAZ_00386596 -->

    <owl:NamedIndividual rdf:about="http://purl.obolibrary.org/obo/GAZ_00386596">
        <obo:RO_0001025 rdf:resource="http://purl.obolibrary.org/obo/GAZ_00042218"/>
        <obo:IAO_0000115>A lake.</obo:IAO_0000115>
        <oboInOwl:hasOBONamespace>GAZ</oboInOwl:hasOBONamespace>
        <oboInOwl:id>GAZ:00386596</oboInOwl:id>
        <rdfs:label>Lacul Racova</rdfs:label>
    </owl:NamedIndividual>
    


    <!-- http://purl.obolibrary.org/obo/GAZ_00386597 -->

    <owl:NamedIndividual rdf:about="http://purl.obolibrary.org/obo/GAZ_00386597">
        <obo:RO_0001025 rdf:resource="http://purl.obolibrary.org/obo/GAZ_00386581"/>
        <obo:IAO_0000115>A lake.</obo:IAO_0000115>
        <oboInOwl:hasOBONamespace>GAZ</oboInOwl:hasOBONamespace>
        <oboInOwl:id>GAZ:00386597</oboInOwl:id>
        <rdfs:label>Lacul Zebil</rdfs:label>
    </owl:NamedIndividual>
    


    <!-- http://purl.obolibrary.org/obo/GAZ_00386598 -->

    <owl:NamedIndividual rdf:about="http://purl.obolibrary.org/obo/GAZ_00386598">
        <obo:RO_0001025 rdf:resource="http://purl.obolibrary.org/obo/GAZ_00042223"/>
        <obo:IAO_0000115>A lake.</obo:IAO_0000115>
        <oboInOwl:hasOBONamespace>GAZ</oboInOwl:hasOBONamespace>
        <oboInOwl:id>GAZ:00386598</oboInOwl:id>
        <rdfs:label>Lacul Ceamurtia</rdfs:label>
    </owl:NamedIndividual>
    


    <!-- http://purl.obolibrary.org/obo/GAZ_00386599 -->

    <owl:NamedIndividual rdf:about="http://purl.obolibrary.org/obo/GAZ_00386599">
        <obo:RO_0001025 rdf:resource="http://purl.obolibrary.org/obo/GAZ_00042218"/>
        <obo:IAO_0000115>A lake.</obo:IAO_0000115>
        <oboInOwl:hasOBONamespace>GAZ</oboInOwl:hasOBONamespace>
        <oboInOwl:id>GAZ:00386599</oboInOwl:id>
        <rdfs:label>Lacul Coseni</rdfs:label>
    </owl:NamedIndividual>
    


    <!-- http://purl.obolibrary.org/obo/GAZ_00386600 -->

    <owl:NamedIndividual rdf:about="http://purl.obolibrary.org/obo/GAZ_00386600">
        <obo:RO_0001025 rdf:resource="http://purl.obolibrary.org/obo/GAZ_00042218"/>
        <obo:IAO_0000115>A lake.</obo:IAO_0000115>
        <oboInOwl:hasOBONamespace>GAZ</oboInOwl:hasOBONamespace>
        <oboInOwl:id>GAZ:00386600</oboInOwl:id>
        <rdfs:label>Lacul Zafono Mic</rdfs:label>
    </owl:NamedIndividual>
    


    <!-- http://purl.obolibrary.org/obo/GAZ_00386601 -->

    <owl:NamedIndividual rdf:about="http://purl.obolibrary.org/obo/GAZ_00386601">
        <obo:RO_0001025 rdf:resource="http://purl.obolibrary.org/obo/GAZ_00042218"/>
        <obo:IAO_0000115>A lake.</obo:IAO_0000115>
        <oboInOwl:hasOBONamespace>GAZ</oboInOwl:hasOBONamespace>
        <oboInOwl:id>GAZ:00386601</oboInOwl:id>
        <rdfs:label>Lacul Zafonu Mare</rdfs:label>
    </owl:NamedIndividual>
    


    <!-- http://purl.obolibrary.org/obo/GAZ_00386602 -->

    <owl:NamedIndividual rdf:about="http://purl.obolibrary.org/obo/GAZ_00386602">
        <obo:RO_0001025 rdf:resource="http://purl.obolibrary.org/obo/GAZ_00042218"/>
        <obo:IAO_0000115>A lake.</obo:IAO_0000115>
        <oboInOwl:hasOBONamespace>GAZ</oboInOwl:hasOBONamespace>
        <oboInOwl:id>GAZ:00386602</oboInOwl:id>
        <rdfs:label>Lacul Lejai</rdfs:label>
    </owl:NamedIndividual>
    


    <!-- http://purl.obolibrary.org/obo/GAZ_00386603 -->

    <owl:NamedIndividual rdf:about="http://purl.obolibrary.org/obo/GAZ_00386603">
        <obo:RO_0001025 rdf:resource="http://purl.obolibrary.org/obo/GAZ_00042218"/>
        <obo:IAO_0000115>A lake.</obo:IAO_0000115>
        <oboInOwl:hasOBONamespace>GAZ</oboInOwl:hasOBONamespace>
        <oboInOwl:id>GAZ:00386603</oboInOwl:id>
        <rdfs:label>Lacul Mandra</rdfs:label>
    </owl:NamedIndividual>
    


    <!-- http://purl.obolibrary.org/obo/GAZ_00386604 -->

    <owl:NamedIndividual rdf:about="http://purl.obolibrary.org/obo/GAZ_00386604">
        <obo:RO_0001025 rdf:resource="http://purl.obolibrary.org/obo/GAZ_00042218"/>
        <obo:IAO_0000115>A lake.</obo:IAO_0000115>
        <oboInOwl:hasOBONamespace>GAZ</oboInOwl:hasOBONamespace>
        <oboInOwl:id>GAZ:00386604</oboInOwl:id>
        <rdfs:label>Lacul Potcoava</rdfs:label>
    </owl:NamedIndividual>
    


    <!-- http://purl.obolibrary.org/obo/GAZ_00386605 -->

    <owl:NamedIndividual rdf:about="http://purl.obolibrary.org/obo/GAZ_00386605">
        <obo:RO_0001025 rdf:resource="http://purl.obolibrary.org/obo/GAZ_00042218"/>
        <obo:IAO_0000115>A lake.</obo:IAO_0000115>
        <oboInOwl:hasOBONamespace>GAZ</oboInOwl:hasOBONamespace>
        <oboInOwl:id>GAZ:00386605</oboInOwl:id>
        <rdfs:label>Lacul Tataru</rdfs:label>
    </owl:NamedIndividual>
    


    <!-- http://purl.obolibrary.org/obo/GAZ_00386606 -->

    <owl:NamedIndividual rdf:about="http://purl.obolibrary.org/obo/GAZ_00386606">
        <obo:RO_0001025 rdf:resource="http://purl.obolibrary.org/obo/GAZ_00042218"/>
        <obo:IAO_0000115>A lake.</obo:IAO_0000115>
        <oboInOwl:hasOBONamespace>GAZ</oboInOwl:hasOBONamespace>
        <oboInOwl:id>GAZ:00386606</oboInOwl:id>
        <rdfs:label>Lacul Bondar</rdfs:label>
    </owl:NamedIndividual>
    


    <!-- http://purl.obolibrary.org/obo/GAZ_00386607 -->

    <owl:NamedIndividual rdf:about="http://purl.obolibrary.org/obo/GAZ_00386607">
        <obo:RO_0001025 rdf:resource="http://purl.obolibrary.org/obo/GAZ_00042218"/>
        <obo:IAO_0000115>A lake.</obo:IAO_0000115>
        <oboInOwl:hasOBONamespace>GAZ</oboInOwl:hasOBONamespace>
        <oboInOwl:id>GAZ:00386607</oboInOwl:id>
        <rdfs:label>Lacul Puiulet</rdfs:label>
    </owl:NamedIndividual>
    


    <!-- http://purl.obolibrary.org/obo/GAZ_00386608 -->

    <owl:NamedIndividual rdf:about="http://purl.obolibrary.org/obo/GAZ_00386608">
        <obo:RO_0001025 rdf:resource="http://purl.obolibrary.org/obo/GAZ_00042218"/>
        <obo:IAO_0000115>A lake.</obo:IAO_0000115>
        <oboInOwl:hasOBONamespace>GAZ</oboInOwl:hasOBONamespace>
        <oboInOwl:id>GAZ:00386608</oboInOwl:id>
        <rdfs:label>Lacul Chiril</rdfs:label>
    </owl:NamedIndividual>
    


    <!-- http://purl.obolibrary.org/obo/GAZ_00386609 -->

    <owl:NamedIndividual rdf:about="http://purl.obolibrary.org/obo/GAZ_00386609">
        <obo:RO_0001025 rdf:resource="http://purl.obolibrary.org/obo/GAZ_00042218"/>
        <obo:IAO_0000115>A lake.</obo:IAO_0000115>
        <oboInOwl:hasOBONamespace>GAZ</oboInOwl:hasOBONamespace>
        <oboInOwl:id>GAZ:00386609</oboInOwl:id>
        <rdfs:label>Lacul Iacob</rdfs:label>
    </owl:NamedIndividual>
    


    <!-- http://purl.obolibrary.org/obo/GAZ_00386610 -->

    <owl:NamedIndividual rdf:about="http://purl.obolibrary.org/obo/GAZ_00386610">
        <obo:RO_0001025 rdf:resource="http://purl.obolibrary.org/obo/GAZ_00042218"/>
        <obo:IAO_0000115>A lake.</obo:IAO_0000115>
        <oboInOwl:hasOBONamespace>GAZ</oboInOwl:hasOBONamespace>
        <oboInOwl:id>GAZ:00386610</oboInOwl:id>
        <rdfs:label>Lacul Taranova</rdfs:label>
    </owl:NamedIndividual>
    


    <!-- http://purl.obolibrary.org/obo/GAZ_00386611 -->

    <owl:NamedIndividual rdf:about="http://purl.obolibrary.org/obo/GAZ_00386611">
        <obo:RO_0001025 rdf:resource="http://purl.obolibrary.org/obo/GAZ_00042218"/>
        <obo:IAO_0000115>A lake.</obo:IAO_0000115>
        <oboInOwl:hasOBONamespace>GAZ</oboInOwl:hasOBONamespace>
        <oboInOwl:id>GAZ:00386611</oboInOwl:id>
        <rdfs:label>Lacul Obtetinciuc</rdfs:label>
    </owl:NamedIndividual>
    


    <!-- http://purl.obolibrary.org/obo/GAZ_00386612 -->

    <owl:NamedIndividual rdf:about="http://purl.obolibrary.org/obo/GAZ_00386612">
        <obo:RO_0001025 rdf:resource="http://purl.obolibrary.org/obo/GAZ_00042218"/>
        <obo:IAO_0000115>A lake.</obo:IAO_0000115>
        <oboInOwl:hasOBONamespace>GAZ</oboInOwl:hasOBONamespace>
        <oboInOwl:id>GAZ:00386612</oboInOwl:id>
        <rdfs:label>Lacul Murighiol</rdfs:label>
    </owl:NamedIndividual>
    


    <!-- http://purl.obolibrary.org/obo/GAZ_00386613 -->

    <owl:NamedIndividual rdf:about="http://purl.obolibrary.org/obo/GAZ_00386613">
        <obo:RO_0001025 rdf:resource="http://purl.obolibrary.org/obo/GAZ_00042218"/>
        <obo:IAO_0000115>A lake.</obo:IAO_0000115>
        <oboInOwl:hasOBONamespace>GAZ</oboInOwl:hasOBONamespace>
        <oboInOwl:id>GAZ:00386613</oboInOwl:id>
        <rdfs:label>Lacul Zaghen</rdfs:label>
    </owl:NamedIndividual>
    


    <!-- http://purl.obolibrary.org/obo/GAZ_00386614 -->

    <owl:NamedIndividual rdf:about="http://purl.obolibrary.org/obo/GAZ_00386614">
        <obo:RO_0001025 rdf:resource="http://purl.obolibrary.org/obo/GAZ_00042218"/>
        <obo:IAO_0000115>A lake.</obo:IAO_0000115>
        <oboInOwl:hasOBONamespace>GAZ</oboInOwl:hasOBONamespace>
        <oboInOwl:id>GAZ:00386614</oboInOwl:id>
        <rdfs:label>Lacul Somova</rdfs:label>
    </owl:NamedIndividual>
    


    <!-- http://purl.obolibrary.org/obo/GAZ_00386615 -->

    <owl:NamedIndividual rdf:about="http://purl.obolibrary.org/obo/GAZ_00386615">
        <obo:RO_0001025 rdf:resource="http://purl.obolibrary.org/obo/GAZ_00042218"/>
        <obo:IAO_0000115>A lake.</obo:IAO_0000115>
        <oboInOwl:hasOBONamespace>GAZ</oboInOwl:hasOBONamespace>
        <oboInOwl:id>GAZ:00386615</oboInOwl:id>
        <rdfs:label>Lacul Obretinu Mare</rdfs:label>
    </owl:NamedIndividual>
    


    <!-- http://purl.obolibrary.org/obo/GAZ_00386616 -->

    <owl:NamedIndividual rdf:about="http://purl.obolibrary.org/obo/GAZ_00386616">
        <obo:RO_0001025 rdf:resource="http://purl.obolibrary.org/obo/GAZ_00042218"/>
        <obo:IAO_0000115>A lake.</obo:IAO_0000115>
        <oboInOwl:hasOBONamespace>GAZ</oboInOwl:hasOBONamespace>
        <oboInOwl:id>GAZ:00386616</oboInOwl:id>
        <rdfs:label>Lacul Obretinu Mica</rdfs:label>
    </owl:NamedIndividual>
    


    <!-- http://purl.obolibrary.org/obo/GAZ_00386617 -->

    <owl:NamedIndividual rdf:about="http://purl.obolibrary.org/obo/GAZ_00386617">
        <obo:RO_0001025 rdf:resource="http://purl.obolibrary.org/obo/GAZ_00042218"/>
        <obo:IAO_0000115>A lake.</obo:IAO_0000115>
        <oboInOwl:hasOBONamespace>GAZ</oboInOwl:hasOBONamespace>
        <oboInOwl:id>GAZ:00386617</oboInOwl:id>
        <rdfs:label>Lacul Vacaru</rdfs:label>
    </owl:NamedIndividual>
    


    <!-- http://purl.obolibrary.org/obo/GAZ_00386618 -->

    <owl:NamedIndividual rdf:about="http://purl.obolibrary.org/obo/GAZ_00386618">
        <obo:RO_0001025 rdf:resource="http://purl.obolibrary.org/obo/GAZ_00042218"/>
        <obo:IAO_0000115>A lake.</obo:IAO_0000115>
        <oboInOwl:hasOBONamespace>GAZ</oboInOwl:hasOBONamespace>
        <oboInOwl:id>GAZ:00386618</oboInOwl:id>
        <rdfs:label>Lacul Ligheanca</rdfs:label>
    </owl:NamedIndividual>
    


    <!-- http://purl.obolibrary.org/obo/GAZ_00386619 -->

    <owl:NamedIndividual rdf:about="http://purl.obolibrary.org/obo/GAZ_00386619">
        <obo:RO_0001025 rdf:resource="http://purl.obolibrary.org/obo/GAZ_00042218"/>
        <obo:IAO_0000115>A lake.</obo:IAO_0000115>
        <oboInOwl:hasOBONamespace>GAZ</oboInOwl:hasOBONamespace>
        <oboInOwl:id>GAZ:00386619</oboInOwl:id>
        <rdfs:label>Lacul Bogdaproste</rdfs:label>
    </owl:NamedIndividual>
    


    <!-- http://purl.obolibrary.org/obo/GAZ_00386620 -->

    <owl:NamedIndividual rdf:about="http://purl.obolibrary.org/obo/GAZ_00386620">
        <obo:RO_0001025 rdf:resource="http://purl.obolibrary.org/obo/GAZ_00042218"/>
        <obo:IAO_0000115>A lake.</obo:IAO_0000115>
        <oboInOwl:hasOBONamespace>GAZ</oboInOwl:hasOBONamespace>
        <oboInOwl:id>GAZ:00386620</oboInOwl:id>
        <rdfs:label>Lacul Babina</rdfs:label>
    </owl:NamedIndividual>
    


    <!-- http://purl.obolibrary.org/obo/GAZ_00386821 -->

    <owl:NamedIndividual rdf:about="http://purl.obolibrary.org/obo/GAZ_00386821">
        <obo:IAO_0000115>A large hydroelectric complex on the Lotru River.</obo:IAO_0000115>
        <oboInOwl:hasOBONamespace>GAZ</oboInOwl:hasOBONamespace>
        <oboInOwl:id>GAZ:00386821</oboInOwl:id>
        <rdfs:label>Lotru-Ciunget Hydroelectric Power Station</rdfs:label>
    </owl:NamedIndividual>
    


    <!-- http://purl.obolibrary.org/obo/GAZ_00387015 -->

    <owl:NamedIndividual rdf:about="http://purl.obolibrary.org/obo/GAZ_00387015">
        <obo:RO_0001025 rdf:resource="http://purl.obolibrary.org/obo/GAZ_00042218"/>
        <obo:IAO_0000115>A protected area. It is located between the Sulina and Chilia branches of Danube in the Danube Delta</obo:IAO_0000115>
        <oboInOwl:hasOBONamespace>GAZ</oboInOwl:hasOBONamespace>
        <oboInOwl:id>GAZ:00387015</oboInOwl:id>
        <rdfs:label>Letea Forest</rdfs:label>
    </owl:NamedIndividual>
    


    <!-- http://purl.obolibrary.org/obo/GAZ_00387017 -->

    <owl:NamedIndividual rdf:about="http://purl.obolibrary.org/obo/GAZ_00387017">
        <obo:RO_0001025 rdf:resource="http://purl.obolibrary.org/obo/GAZ_00387018"/>
        <obo:IAO_0000115>A protected area.</obo:IAO_0000115>
        <oboInOwl:hasOBONamespace>GAZ</oboInOwl:hasOBONamespace>
        <oboInOwl:id>GAZ:00387017</oboInOwl:id>
        <rdfs:label>Parcul National Piatra Craiului</rdfs:label>
    </owl:NamedIndividual>
    


    <!-- http://purl.obolibrary.org/obo/GAZ_00387018 -->

    <owl:NamedIndividual rdf:about="http://purl.obolibrary.org/obo/GAZ_00387018">
        <obo:RO_0001025 rdf:resource="http://purl.obolibrary.org/obo/GAZ_00061983"/>
        <obo:IAO_0000115>A mountain range in the Southern Carpathians in Romania. The massif is bordered in the west by the Dambovita Valley which separates it from the Papusa massif; in the north-west the river Barsa and Curmatura Foii separates it from the Fagaras Mountains and in the east the &quot;Bran-Rucar passage&quot; delimits it from the Bucegi and Leaota mountains. The southern border is the confluence of the valleys of Dambovita and Dambovicioara rivers, in the &quot;Podul Dambovitei&quot; depression.</obo:IAO_0000115>
        <oboInOwl:hasOBONamespace>GAZ</oboInOwl:hasOBONamespace>
        <oboInOwl:id>GAZ:00387018</oboInOwl:id>
        <rdfs:label>Muntii Piatra Craiului</rdfs:label>
    </owl:NamedIndividual>
    


    <!-- http://purl.obolibrary.org/obo/GAZ_00387019 -->

    <owl:NamedIndividual rdf:about="http://purl.obolibrary.org/obo/GAZ_00387019">
        <obo:RO_0001025 rdf:resource="http://purl.obolibrary.org/obo/GAZ_00062036"/>
        <obo:IAO_0000115>A protected area.</obo:IAO_0000115>
        <oboInOwl:hasOBONamespace>GAZ</oboInOwl:hasOBONamespace>
        <oboInOwl:id>GAZ:00387019</oboInOwl:id>
        <rdfs:label>Parcul National Semenic</rdfs:label>
    </owl:NamedIndividual>
    


    <!-- http://purl.obolibrary.org/obo/GAZ_00387020 -->

    <owl:NamedIndividual rdf:about="http://purl.obolibrary.org/obo/GAZ_00387020">
        <obo:RO_0001025 rdf:resource="http://purl.obolibrary.org/obo/GAZ_00061981"/>
        <obo:IAO_0000115>A protected area.</obo:IAO_0000115>
        <oboInOwl:hasOBONamespace>GAZ</oboInOwl:hasOBONamespace>
        <oboInOwl:id>GAZ:00387020</oboInOwl:id>
        <rdfs:label>Parcul National Muntii Rodnei</rdfs:label>
    </owl:NamedIndividual>
    


    <!-- http://purl.obolibrary.org/obo/GAZ_00387021 -->

    <owl:NamedIndividual rdf:about="http://purl.obolibrary.org/obo/GAZ_00387021">
        <obo:RO_0001025 rdf:resource="http://purl.obolibrary.org/obo/GAZ_00387020"/>
        <obo:IAO_0000115>A protected area.</obo:IAO_0000115>
        <oboInOwl:hasOBONamespace>GAZ</oboInOwl:hasOBONamespace>
        <oboInOwl:id>GAZ:00387021</oboInOwl:id>
        <rdfs:label>Rezervatia stiintifica Pietrosu Mare</rdfs:label>
    </owl:NamedIndividual>
    


    <!-- http://purl.obolibrary.org/obo/GAZ_00387022 -->

    <owl:NamedIndividual rdf:about="http://purl.obolibrary.org/obo/GAZ_00387022">
        <obo:RO_0001025 rdf:resource="http://purl.obolibrary.org/obo/GAZ_00387020"/>
        <obo:IAO_0000115>A protected area.</obo:IAO_0000115>
        <oboInOwl:hasOBONamespace>GAZ</oboInOwl:hasOBONamespace>
        <oboInOwl:id>GAZ:00387022</oboInOwl:id>
        <rdfs:label>Rezervatia stiintifica Piatra Rea</rdfs:label>
    </owl:NamedIndividual>
    


    <!-- http://purl.obolibrary.org/obo/GAZ_00387023 -->

    <owl:NamedIndividual rdf:about="http://purl.obolibrary.org/obo/GAZ_00387023">
        <obo:RO_0001025 rdf:resource="http://purl.obolibrary.org/obo/GAZ_00387020"/>
        <obo:IAO_0000115>A protected area.</obo:IAO_0000115>
        <oboInOwl:hasOBONamespace>GAZ</oboInOwl:hasOBONamespace>
        <oboInOwl:id>GAZ:00387023</oboInOwl:id>
        <rdfs:label>Rezervatia mixta Pestera si Izbucul Izvorul Albastru al Izei</rdfs:label>
    </owl:NamedIndividual>
    


    <!-- http://purl.obolibrary.org/obo/GAZ_00387024 -->

    <owl:NamedIndividual rdf:about="http://purl.obolibrary.org/obo/GAZ_00387024">
        <obo:RO_0001025 rdf:resource="http://purl.obolibrary.org/obo/GAZ_00387020"/>
        <obo:IAO_0000115>A protected area.</obo:IAO_0000115>
        <oboInOwl:hasOBONamespace>GAZ</oboInOwl:hasOBONamespace>
        <oboInOwl:id>GAZ:00387024</oboInOwl:id>
        <rdfs:label>Rezervatia botanica Poiana cu narcise din Muntele Saca</rdfs:label>
    </owl:NamedIndividual>
    


    <!-- http://purl.obolibrary.org/obo/GAZ_00387025 -->

    <owl:NamedIndividual rdf:about="http://purl.obolibrary.org/obo/GAZ_00387025">
        <obo:RO_0001025 rdf:resource="http://purl.obolibrary.org/obo/GAZ_00387020"/>
        <obo:IAO_0000115>A protected area.</obo:IAO_0000115>
        <oboInOwl:hasOBONamespace>GAZ</oboInOwl:hasOBONamespace>
        <oboInOwl:id>GAZ:00387025</oboInOwl:id>
        <rdfs:label>Rezervatia speologica Pestera Cobasel</rdfs:label>
    </owl:NamedIndividual>
    


    <!-- http://purl.obolibrary.org/obo/GAZ_00387026 -->

    <owl:NamedIndividual rdf:about="http://purl.obolibrary.org/obo/GAZ_00387026">
        <obo:RO_0001025 rdf:resource="http://purl.obolibrary.org/obo/GAZ_00387020"/>
        <obo:IAO_0000115>A protected area.</obo:IAO_0000115>
        <oboInOwl:hasOBONamespace>GAZ</oboInOwl:hasOBONamespace>
        <oboInOwl:id>GAZ:00387026</oboInOwl:id>
        <rdfs:label>Rezervatia mixta Ineu - Lala</rdfs:label>
    </owl:NamedIndividual>
    


    <!-- http://purl.obolibrary.org/obo/GAZ_00387027 -->

    <owl:NamedIndividual rdf:about="http://purl.obolibrary.org/obo/GAZ_00387027">
        <obo:RO_0001025 rdf:resource="http://purl.obolibrary.org/obo/GAZ_00387020"/>
        <obo:IAO_0000115>A protected area.</obo:IAO_0000115>
        <oboInOwl:hasOBONamespace>GAZ</oboInOwl:hasOBONamespace>
        <oboInOwl:id>GAZ:00387027</oboInOwl:id>
        <rdfs:label>Rezervatia naturala Pestera de la Izvorul Tausoarelor</rdfs:label>
    </owl:NamedIndividual>
    


    <!-- http://purl.obolibrary.org/obo/GAZ_00387028 -->

    <owl:NamedIndividual rdf:about="http://purl.obolibrary.org/obo/GAZ_00387028">
        <obo:RO_0001025 rdf:resource="http://purl.obolibrary.org/obo/GAZ_00387020"/>
        <obo:IAO_0000115>A protected area.</obo:IAO_0000115>
        <oboInOwl:hasOBONamespace>GAZ</oboInOwl:hasOBONamespace>
        <oboInOwl:id>GAZ:00387028</oboInOwl:id>
        <rdfs:label>Rezervatia naturala Izvorul Batrana</rdfs:label>
    </owl:NamedIndividual>
    


    <!-- http://purl.obolibrary.org/obo/GAZ_00387029 -->

    <owl:NamedIndividual rdf:about="http://purl.obolibrary.org/obo/GAZ_00387029">
        <obo:RO_0001025 rdf:resource="http://purl.obolibrary.org/obo/GAZ_00387020"/>
        <obo:IAO_0000115>A protected area.</obo:IAO_0000115>
        <oboInOwl:hasOBONamespace>GAZ</oboInOwl:hasOBONamespace>
        <oboInOwl:id>GAZ:00387029</oboInOwl:id>
        <rdfs:label>Rezervatia mixta Izvoarele Mihaiesei</rdfs:label>
    </owl:NamedIndividual>
    


    <!-- http://purl.obolibrary.org/obo/GAZ_00387030 -->

    <owl:NamedIndividual rdf:about="http://purl.obolibrary.org/obo/GAZ_00387030">
        <obo:RO_0001025 rdf:resource="http://purl.obolibrary.org/obo/GAZ_00387021"/>
        <obo:IAO_0000115>A glacial lake.</obo:IAO_0000115>
        <oboInOwl:hasOBONamespace>GAZ</oboInOwl:hasOBONamespace>
        <oboInOwl:id>GAZ:00387030</oboInOwl:id>
        <rdfs:label>Buhaescu IV</rdfs:label>
    </owl:NamedIndividual>
    


    <!-- http://purl.obolibrary.org/obo/GAZ_00387032 -->

    <owl:NamedIndividual rdf:about="http://purl.obolibrary.org/obo/GAZ_00387032">
        <obo:RO_0001025 rdf:resource="http://purl.obolibrary.org/obo/GAZ_00062011"/>
        <obo:IAO_0000115>A cave.</obo:IAO_0000115>
        <oboInOwl:hasOBONamespace>GAZ</oboInOwl:hasOBONamespace>
        <oboInOwl:id>GAZ:00387032</oboInOwl:id>
        <rdfs:label>Pestera Fugarilor</rdfs:label>
    </owl:NamedIndividual>
    


    <!-- http://purl.obolibrary.org/obo/GAZ_00387038 -->

    <owl:NamedIndividual rdf:about="http://purl.obolibrary.org/obo/GAZ_00387038">
        <obo:RO_0001025 rdf:resource="http://purl.obolibrary.org/obo/GAZ_00061995"/>
        <obo:IAO_0000115>A protected area.</obo:IAO_0000115>
        <oboInOwl:hasOBONamespace>GAZ</oboInOwl:hasOBONamespace>
        <oboInOwl:id>GAZ:00387038</oboInOwl:id>
        <rdfs:label>Parcul National Cozia</rdfs:label>
    </owl:NamedIndividual>
    


    <!-- http://purl.obolibrary.org/obo/GAZ_00387039 -->

    <owl:NamedIndividual rdf:about="http://purl.obolibrary.org/obo/GAZ_00387039">
        <obo:RO_0001025 rdf:resource="http://purl.obolibrary.org/obo/GAZ_00061970"/>
        <obo:IAO_0000115>A protected area.</obo:IAO_0000115>
        <oboInOwl:hasOBONamespace>GAZ</oboInOwl:hasOBONamespace>
        <oboInOwl:id>GAZ:00387039</oboInOwl:id>
        <rdfs:label>Parcul National Calimani</rdfs:label>
    </owl:NamedIndividual>
    


    <!-- http://purl.obolibrary.org/obo/GAZ_00387040 -->

    <owl:NamedIndividual rdf:about="http://purl.obolibrary.org/obo/GAZ_00387040">
        <obo:RO_0001025 rdf:resource="http://purl.obolibrary.org/obo/GAZ_00387039"/>
        <obo:IAO_0000115>A protected area.</obo:IAO_0000115>
        <oboInOwl:hasOBONamespace>GAZ</oboInOwl:hasOBONamespace>
        <oboInOwl:id>GAZ:00387040</oboInOwl:id>
        <rdfs:label>Rezervatia Stiintifica de Jnepenis cu Pinus cembra</rdfs:label>
    </owl:NamedIndividual>
    


    <!-- http://purl.obolibrary.org/obo/GAZ_00387041 -->

    <owl:NamedIndividual rdf:about="http://purl.obolibrary.org/obo/GAZ_00387041">
        <obo:RO_0001025 rdf:resource="http://purl.obolibrary.org/obo/GAZ_00387039"/>
        <obo:IAO_0000115>A protected area.</obo:IAO_0000115>
        <oboInOwl:hasOBONamespace>GAZ</oboInOwl:hasOBONamespace>
        <oboInOwl:id>GAZ:00387041</oboInOwl:id>
        <rdfs:label>Rezervatia Lacul Iezer</rdfs:label>
    </owl:NamedIndividual>
    


    <!-- http://purl.obolibrary.org/obo/GAZ_00387042 -->

    <owl:NamedIndividual rdf:about="http://purl.obolibrary.org/obo/GAZ_00387042">
        <obo:RO_0001025 rdf:resource="http://purl.obolibrary.org/obo/GAZ_00387039"/>
        <obo:IAO_0000115>A protected area.</obo:IAO_0000115>
        <oboInOwl:hasOBONamespace>GAZ</oboInOwl:hasOBONamespace>
        <oboInOwl:id>GAZ:00387042</oboInOwl:id>
        <rdfs:label>Rezervatia geologica 12 Apostoli</rdfs:label>
    </owl:NamedIndividual>
    


    <!-- http://purl.obolibrary.org/obo/GAZ_00387043 -->

    <owl:NamedIndividual rdf:about="http://purl.obolibrary.org/obo/GAZ_00387043">
        <obo:RO_0001025 rdf:resource="http://purl.obolibrary.org/obo/GAZ_00061705"/>
        <obo:IAO_0000115>A protected area.</obo:IAO_0000115>
        <oboInOwl:hasOBONamespace>GAZ</oboInOwl:hasOBONamespace>
        <oboInOwl:id>GAZ:00387043</oboInOwl:id>
        <rdfs:label>Parcul Natural Apuseni</rdfs:label>
    </owl:NamedIndividual>
    


    <!-- http://purl.obolibrary.org/obo/GAZ_00387044 -->

    <owl:NamedIndividual rdf:about="http://purl.obolibrary.org/obo/GAZ_00387044">
        <obo:RO_0001025 rdf:resource="http://purl.obolibrary.org/obo/GAZ_00061987"/>
        <obo:IAO_0000115>A protected area.</obo:IAO_0000115>
        <oboInOwl:hasOBONamespace>GAZ</oboInOwl:hasOBONamespace>
        <oboInOwl:id>GAZ:00387044</oboInOwl:id>
        <rdfs:label>Parcul Natural Gradistea Muncelului-Cioclovina</rdfs:label>
    </owl:NamedIndividual>
    


    <!-- http://purl.obolibrary.org/obo/GAZ_00387050 -->

    <owl:NamedIndividual rdf:about="http://purl.obolibrary.org/obo/GAZ_00387050">
        <obo:RO_0001025 rdf:resource="http://purl.obolibrary.org/obo/GAZ_00062025"/>
        <obo:IAO_0000115>A protected area.</obo:IAO_0000115>
        <oboInOwl:hasOBONamespace>GAZ</oboInOwl:hasOBONamespace>
        <oboInOwl:id>GAZ:00387050</oboInOwl:id>
        <rdfs:label>Rezervatia Naturala Cheile Intregalde</rdfs:label>
    </owl:NamedIndividual>
    


    <!-- http://purl.obolibrary.org/obo/GAZ_00387051 -->

    <owl:NamedIndividual rdf:about="http://purl.obolibrary.org/obo/GAZ_00387051">
        <obo:RO_0001025 rdf:resource="http://purl.obolibrary.org/obo/GAZ_00062025"/>
        <obo:IAO_0000115>A protected area.</obo:IAO_0000115>
        <oboInOwl:hasOBONamespace>GAZ</oboInOwl:hasOBONamespace>
        <oboInOwl:id>GAZ:00387051</oboInOwl:id>
        <rdfs:label>Rezervatia Naturala Cheile Rametului</rdfs:label>
    </owl:NamedIndividual>
    


    <!-- http://purl.obolibrary.org/obo/GAZ_00387053 -->

    <owl:NamedIndividual rdf:about="http://purl.obolibrary.org/obo/GAZ_00387053">
        <obo:RO_0001025 rdf:resource="http://purl.obolibrary.org/obo/GAZ_00062025"/>
        <obo:IAO_0000115>A protected area.</obo:IAO_0000115>
        <oboInOwl:hasOBONamespace>GAZ</oboInOwl:hasOBONamespace>
        <oboInOwl:id>GAZ:00387053</oboInOwl:id>
        <rdfs:label>Rezervatia Naturala Huda lui Papara</rdfs:label>
    </owl:NamedIndividual>
    


    <!-- http://purl.obolibrary.org/obo/GAZ_00387054 -->

    <owl:NamedIndividual rdf:about="http://purl.obolibrary.org/obo/GAZ_00387054">
        <obo:RO_0001025 rdf:resource="http://purl.obolibrary.org/obo/GAZ_00062025"/>
        <obo:IAO_0000115>A protected area.</obo:IAO_0000115>
        <oboInOwl:hasOBONamespace>GAZ</oboInOwl:hasOBONamespace>
        <oboInOwl:id>GAZ:00387054</oboInOwl:id>
        <rdfs:label>Rezervatia Naturala Cheile Manastirii</rdfs:label>
    </owl:NamedIndividual>
    


    <!-- http://purl.obolibrary.org/obo/GAZ_00387081 -->

    <owl:NamedIndividual rdf:about="http://purl.obolibrary.org/obo/GAZ_00387081">
        <obo:IAO_0000115>An island. Located just downstream of the city of Turnu Severin and overlooking the town of Simian.</obo:IAO_0000115>
        <oboInOwl:hasOBONamespace>GAZ</oboInOwl:hasOBONamespace>
        <oboInOwl:id>GAZ:00387081</oboInOwl:id>
        <rdfs:label>Simian</rdfs:label>
    </owl:NamedIndividual>
    


    <!-- http://purl.obolibrary.org/obo/GAZ_00387082 -->

    <owl:NamedIndividual rdf:about="http://purl.obolibrary.org/obo/GAZ_00387082">
        <obo:RO_0001025 rdf:resource="http://purl.obolibrary.org/obo/GAZ_00061698"/>
        <obo:IAO_0000115>A mountain range. They run from the Azuga Valley in the North and to the Posada Gorges in the South, and from the Doftana Valley in the East to the Prahova Valley in the West.</obo:IAO_0000115>
        <oboInOwl:hasOBONamespace>GAZ</oboInOwl:hasOBONamespace>
        <oboInOwl:id>GAZ:00387082</oboInOwl:id>
        <rdfs:label>Baiu Mountains</rdfs:label>
    </owl:NamedIndividual>
    


    <!-- http://purl.obolibrary.org/obo/GAZ_00387083 -->

    <owl:NamedIndividual rdf:about="http://purl.obolibrary.org/obo/GAZ_00387083">
        <obo:RO_0001025 rdf:resource="http://purl.obolibrary.org/obo/GAZ_00061698"/>
        <obo:IAO_0000115>A mountain range.</obo:IAO_0000115>
        <oboInOwl:hasOBONamespace>GAZ</oboInOwl:hasOBONamespace>
        <oboInOwl:id>GAZ:00387083</oboInOwl:id>
        <rdfs:label>Carpatii de Curbura</rdfs:label>
    </owl:NamedIndividual>
    


    <!-- http://purl.obolibrary.org/obo/GAZ_00387084 -->

    <owl:NamedIndividual rdf:about="http://purl.obolibrary.org/obo/GAZ_00387084">
        <obo:RO_0001025 rdf:resource="http://purl.obolibrary.org/obo/GAZ_00387083"/>
        <obo:IAO_0000115>A mountain massif.</obo:IAO_0000115>
        <oboInOwl:hasOBONamespace>GAZ</oboInOwl:hasOBONamespace>
        <oboInOwl:id>GAZ:00387084</oboInOwl:id>
        <rdfs:label>Masivul Postavarul</rdfs:label>
    </owl:NamedIndividual>
    


    <!-- http://purl.obolibrary.org/obo/GAZ_00387086 -->

    <owl:NamedIndividual rdf:about="http://purl.obolibrary.org/obo/GAZ_00387086">
        <obo:RO_0001025 rdf:resource="http://purl.obolibrary.org/obo/GAZ_00387026"/>
        <obo:IAO_0000115>A glacial lake.</obo:IAO_0000115>
        <oboInOwl:hasOBONamespace>GAZ</oboInOwl:hasOBONamespace>
        <oboInOwl:id>GAZ:00387086</oboInOwl:id>
        <rdfs:label>Lacul Lala Mic</rdfs:label>
    </owl:NamedIndividual>
    


    <!-- http://purl.obolibrary.org/obo/GAZ_00387093 -->

    <owl:NamedIndividual rdf:about="http://purl.obolibrary.org/obo/GAZ_00387093">
        <obo:RO_0001025 rdf:resource="http://purl.obolibrary.org/obo/GAZ_00061970"/>
        <obo:IAO_0000115>A reservoir.</obo:IAO_0000115>
        <oboInOwl:hasOBONamespace>GAZ</oboInOwl:hasOBONamespace>
        <oboInOwl:id>GAZ:00387093</oboInOwl:id>
        <rdfs:label>Lacul Colibita</rdfs:label>
    </owl:NamedIndividual>
    


    <!-- http://purl.obolibrary.org/obo/GAZ_00387094 -->

    <owl:NamedIndividual rdf:about="http://purl.obolibrary.org/obo/GAZ_00387094">
        <obo:RO_0001025 rdf:resource="http://purl.obolibrary.org/obo/GAZ_00061905"/>
        <obo:IAO_0000115>A mountain range.</obo:IAO_0000115>
        <oboInOwl:hasOBONamespace>GAZ</oboInOwl:hasOBONamespace>
        <oboInOwl:id>GAZ:00387094</oboInOwl:id>
        <rdfs:label>Obcina Feredeu</rdfs:label>
    </owl:NamedIndividual>
    


    <!-- http://purl.obolibrary.org/obo/GAZ_00387095 -->

    <owl:NamedIndividual rdf:about="http://purl.obolibrary.org/obo/GAZ_00387095">
        <obo:RO_0001025 rdf:resource="http://purl.obolibrary.org/obo/GAZ_00387094"/>
        <obo:IAO_0000115>A lake.</obo:IAO_0000115>
        <oboInOwl:hasOBONamespace>GAZ</oboInOwl:hasOBONamespace>
        <oboInOwl:id>GAZ:00387095</oboInOwl:id>
        <rdfs:label>Sadova</rdfs:label>
    </owl:NamedIndividual>
    


    <!-- http://purl.obolibrary.org/obo/GAZ_00387096 -->

    <owl:NamedIndividual rdf:about="http://purl.obolibrary.org/obo/GAZ_00387096">
        <obo:RO_0001025 rdf:resource="http://purl.obolibrary.org/obo/GAZ_00061950"/>
        <obo:IAO_0000115>A reservoir.</obo:IAO_0000115>
        <oboInOwl:hasOBONamespace>GAZ</oboInOwl:hasOBONamespace>
        <oboInOwl:id>GAZ:00387096</oboInOwl:id>
        <rdfs:label>Lacul Sacele</rdfs:label>
    </owl:NamedIndividual>
    


    <!-- http://purl.obolibrary.org/obo/GAZ_00387097 -->

    <owl:NamedIndividual rdf:about="http://purl.obolibrary.org/obo/GAZ_00387097">
        <obo:RO_0001025 rdf:resource="http://purl.obolibrary.org/obo/GAZ_00062922"/>
        <obo:IAO_0000115>A glacial lake.</obo:IAO_0000115>
        <oboInOwl:hasOBONamespace>GAZ</oboInOwl:hasOBONamespace>
        <oboInOwl:id>GAZ:00387097</oboInOwl:id>
        <rdfs:label>Galbena II</rdfs:label>
    </owl:NamedIndividual>
    


    <!-- http://purl.obolibrary.org/obo/GAZ_00387098 -->

    <owl:NamedIndividual rdf:about="http://purl.obolibrary.org/obo/GAZ_00387098">
        <obo:RO_0001025 rdf:resource="http://purl.obolibrary.org/obo/GAZ_00062922"/>
        <obo:IAO_0000115>A glacial lake.</obo:IAO_0000115>
        <oboInOwl:hasOBONamespace>GAZ</oboInOwl:hasOBONamespace>
        <oboInOwl:id>GAZ:00387098</oboInOwl:id>
        <rdfs:label>Galbena III</rdfs:label>
    </owl:NamedIndividual>
    


    <!-- http://purl.obolibrary.org/obo/GAZ_00387099 -->

    <owl:NamedIndividual rdf:about="http://purl.obolibrary.org/obo/GAZ_00387099">
        <obo:RO_0001025 rdf:resource="http://purl.obolibrary.org/obo/GAZ_00062922"/>
        <obo:IAO_0000115>A glacial lake.</obo:IAO_0000115>
        <oboInOwl:hasOBONamespace>GAZ</oboInOwl:hasOBONamespace>
        <oboInOwl:id>GAZ:00387099</oboInOwl:id>
        <rdfs:label>Galbena IV</rdfs:label>
    </owl:NamedIndividual>
    


    <!-- http://purl.obolibrary.org/obo/GAZ_00387100 -->

    <owl:NamedIndividual rdf:about="http://purl.obolibrary.org/obo/GAZ_00387100">
        <obo:RO_0001025 rdf:resource="http://purl.obolibrary.org/obo/GAZ_00387019"/>
        <obo:IAO_0000115>A mountain range.</obo:IAO_0000115>
        <oboInOwl:hasOBONamespace>GAZ</oboInOwl:hasOBONamespace>
        <oboInOwl:id>GAZ:00387100</oboInOwl:id>
        <rdfs:label>Muntii Semenic</rdfs:label>
    </owl:NamedIndividual>
    


    <!-- http://purl.obolibrary.org/obo/GAZ_00387101 -->

    <owl:NamedIndividual rdf:about="http://purl.obolibrary.org/obo/GAZ_00387101">
        <obo:RO_0001025 rdf:resource="http://purl.obolibrary.org/obo/GAZ_00387100"/>
        <obo:IAO_0000115>A lake.</obo:IAO_0000115>
        <oboInOwl:hasOBONamespace>GAZ</oboInOwl:hasOBONamespace>
        <oboInOwl:id>GAZ:00387101</oboInOwl:id>
        <rdfs:label>Izvorul Baia Vulturilor</rdfs:label>
    </owl:NamedIndividual>
    


    <!-- http://purl.obolibrary.org/obo/GAZ_00387104 -->

    <owl:NamedIndividual rdf:about="http://purl.obolibrary.org/obo/GAZ_00387104">
        <obo:RO_0001025 rdf:resource="http://purl.obolibrary.org/obo/GAZ_00061983"/>
        <obo:IAO_0000115>A mountain pass.</obo:IAO_0000115>
        <oboInOwl:hasOBONamespace>GAZ</oboInOwl:hasOBONamespace>
        <oboInOwl:id>GAZ:00387104</oboInOwl:id>
        <rdfs:label>Culoarul Bran-Rucar-Dragoslavele</rdfs:label>
    </owl:NamedIndividual>
    


    <!-- http://purl.obolibrary.org/obo/GAZ_00387105 -->

    <owl:NamedIndividual rdf:about="http://purl.obolibrary.org/obo/GAZ_00387105">
        <obo:RO_0001025 rdf:resource="http://purl.obolibrary.org/obo/GAZ_00387104"/>
        <obo:IAO_0000115>A karst depression.</obo:IAO_0000115>
        <oboInOwl:hasOBONamespace>GAZ</oboInOwl:hasOBONamespace>
        <oboInOwl:id>GAZ:00387105</oboInOwl:id>
        <rdfs:label>Depresiunea Dambovicioara</rdfs:label>
    </owl:NamedIndividual>
    


    <!-- http://purl.obolibrary.org/obo/GAZ_00387106 -->

    <owl:NamedIndividual rdf:about="http://purl.obolibrary.org/obo/GAZ_00387106">
        <obo:RO_0001025 rdf:resource="http://purl.obolibrary.org/obo/GAZ_00387104"/>
        <obo:IAO_0000115>A karst depression.</obo:IAO_0000115>
        <oboInOwl:hasOBONamespace>GAZ</oboInOwl:hasOBONamespace>
        <oboInOwl:id>GAZ:00387106</oboInOwl:id>
        <rdfs:label>Depresiunea Rucar</rdfs:label>
    </owl:NamedIndividual>
    


    <!-- http://purl.obolibrary.org/obo/GAZ_00387107 -->

    <owl:NamedIndividual rdf:about="http://purl.obolibrary.org/obo/GAZ_00387107">
        <obo:RO_0001025 rdf:resource="http://purl.obolibrary.org/obo/GAZ_00387104"/>
        <obo:IAO_0000115>A karst depression.</obo:IAO_0000115>
        <oboInOwl:hasOBONamespace>GAZ</oboInOwl:hasOBONamespace>
        <oboInOwl:id>GAZ:00387107</oboInOwl:id>
        <rdfs:label>Depresiunea Podul Dambovitei</rdfs:label>
    </owl:NamedIndividual>
    


    <!-- http://purl.obolibrary.org/obo/GAZ_00387108 -->

    <owl:NamedIndividual rdf:about="http://purl.obolibrary.org/obo/GAZ_00387108">
        <rdf:type rdf:resource="http://purl.obolibrary.org/obo/ENVO_00000100"/>
        <obo:RO_0001025 rdf:resource="http://purl.obolibrary.org/obo/GAZ_00062002"/>
        <obo:IAO_0000115>A gorge.</obo:IAO_0000115>
        <oboInOwl:hasOBONamespace>GAZ</oboInOwl:hasOBONamespace>
        <oboInOwl:id>GAZ:00387108</oboInOwl:id>
        <rdfs:label>Cheile Corcoaia</rdfs:label>
    </owl:NamedIndividual>
    


    <!-- http://purl.obolibrary.org/obo/GAZ_00387109 -->

    <owl:NamedIndividual rdf:about="http://purl.obolibrary.org/obo/GAZ_00387109">
        <rdf:type rdf:resource="http://purl.obolibrary.org/obo/ENVO_00000100"/>
        <obo:RO_0001025 rdf:resource="http://purl.obolibrary.org/obo/GAZ_00387044"/>
        <obo:IAO_0000115>A gorge.</obo:IAO_0000115>
        <oboInOwl:hasOBONamespace>GAZ</oboInOwl:hasOBONamespace>
        <oboInOwl:id>GAZ:00387109</oboInOwl:id>
        <rdfs:label>Cheile Crivadiei</rdfs:label>
    </owl:NamedIndividual>
    


    <!-- http://purl.obolibrary.org/obo/GAZ_00387110 -->

    <owl:NamedIndividual rdf:about="http://purl.obolibrary.org/obo/GAZ_00387110">
        <rdf:type rdf:resource="http://purl.obolibrary.org/obo/ENVO_00000100"/>
        <obo:RO_0001025 rdf:resource="http://purl.obolibrary.org/obo/GAZ_00387018"/>
        <obo:IAO_0000115>A gorge.</obo:IAO_0000115>
        <oboInOwl:hasOBONamespace>GAZ</oboInOwl:hasOBONamespace>
        <oboInOwl:id>GAZ:00387110</oboInOwl:id>
        <rdfs:label>Cheile Dambovicioarei</rdfs:label>
    </owl:NamedIndividual>
    


    <!-- http://purl.obolibrary.org/obo/GAZ_00387111 -->

    <owl:NamedIndividual rdf:about="http://purl.obolibrary.org/obo/GAZ_00387111">
        <rdf:type rdf:resource="http://purl.obolibrary.org/obo/ENVO_00000100"/>
        <obo:RO_0001025 rdf:resource="http://purl.obolibrary.org/obo/GAZ_00062038"/>
        <obo:IAO_0000115>A gorge.</obo:IAO_0000115>
        <oboInOwl:hasOBONamespace>GAZ</oboInOwl:hasOBONamespace>
        <oboInOwl:id>GAZ:00387111</oboInOwl:id>
        <rdfs:label>Cheile Minisului</rdfs:label>
    </owl:NamedIndividual>
    


    <!-- http://purl.obolibrary.org/obo/GAZ_00387112 -->

    <owl:NamedIndividual rdf:about="http://purl.obolibrary.org/obo/GAZ_00387112">
        <rdf:type rdf:resource="http://purl.obolibrary.org/obo/ENVO_00000100"/>
        <obo:RO_0001025 rdf:resource="http://purl.obolibrary.org/obo/GAZ_00062021"/>
        <obo:IAO_0000115>A gorge.</obo:IAO_0000115>
        <oboInOwl:hasOBONamespace>GAZ</oboInOwl:hasOBONamespace>
        <oboInOwl:id>GAZ:00387112</oboInOwl:id>
        <rdfs:label>Cheile Pociovalistei</rdfs:label>
    </owl:NamedIndividual>
    


    <!-- http://purl.obolibrary.org/obo/GAZ_00387113 -->

    <owl:NamedIndividual rdf:about="http://purl.obolibrary.org/obo/GAZ_00387113">
        <obo:IAO_0000115>A protected area.</obo:IAO_0000115>
        <oboInOwl:hasOBONamespace>GAZ</oboInOwl:hasOBONamespace>
        <oboInOwl:id>GAZ:00387113</oboInOwl:id>
        <rdfs:label>Rezervatia de zada de la Vidolm</rdfs:label>
    </owl:NamedIndividual>
    


    <!-- http://purl.obolibrary.org/obo/GAZ_00387114 -->

    <owl:NamedIndividual rdf:about="http://purl.obolibrary.org/obo/GAZ_00387114">
        <rdf:type rdf:resource="http://purl.obolibrary.org/obo/ENVO_00000100"/>
        <obo:RO_0001025 rdf:resource="http://purl.obolibrary.org/obo/GAZ_00062021"/>
        <obo:IAO_0000115>A gorge.</obo:IAO_0000115>
        <oboInOwl:hasOBONamespace>GAZ</oboInOwl:hasOBONamespace>
        <oboInOwl:id>GAZ:00387114</oboInOwl:id>
        <rdfs:label>Cheile Posagii</rdfs:label>
    </owl:NamedIndividual>
    


    <!-- http://purl.obolibrary.org/obo/GAZ_00387116 -->

    <owl:NamedIndividual rdf:about="http://purl.obolibrary.org/obo/GAZ_00387116">
        <rdf:type rdf:resource="http://purl.obolibrary.org/obo/ENVO_00000100"/>
        <obo:RO_0001025 rdf:resource="http://purl.obolibrary.org/obo/GAZ_00061705"/>
        <obo:IAO_0000115>A gorge.</obo:IAO_0000115>
        <oboInOwl:hasOBONamespace>GAZ</oboInOwl:hasOBONamespace>
        <oboInOwl:id>GAZ:00387116</oboInOwl:id>
        <rdfs:label>Cheile Runcului</rdfs:label>
    </owl:NamedIndividual>
    


    <!-- http://purl.obolibrary.org/obo/GAZ_00387117 -->

    <owl:NamedIndividual rdf:about="http://purl.obolibrary.org/obo/GAZ_00387117">
        <rdf:type rdf:resource="http://purl.obolibrary.org/obo/ENVO_00000100"/>
        <obo:RO_0001025 rdf:resource="http://purl.obolibrary.org/obo/GAZ_00061705"/>
        <obo:IAO_0000115>A gorge.</obo:IAO_0000115>
        <oboInOwl:hasOBONamespace>GAZ</oboInOwl:hasOBONamespace>
        <oboInOwl:id>GAZ:00387117</oboInOwl:id>
        <rdfs:label>Cheile Rametilor</rdfs:label>
    </owl:NamedIndividual>
    


    <!-- http://purl.obolibrary.org/obo/GAZ_00387119 -->

    <owl:NamedIndividual rdf:about="http://purl.obolibrary.org/obo/GAZ_00387119">
        <rdf:type rdf:resource="http://purl.obolibrary.org/obo/ENVO_00000100"/>
        <obo:RO_0001025 rdf:resource="http://purl.obolibrary.org/obo/GAZ_00061961"/>
        <obo:IAO_0000115>A gorge.</obo:IAO_0000115>
        <oboInOwl:hasOBONamespace>GAZ</oboInOwl:hasOBONamespace>
        <oboInOwl:id>GAZ:00387119</oboInOwl:id>
        <rdfs:label>Cheile Tatarului</rdfs:label>
    </owl:NamedIndividual>
    


    <!-- http://purl.obolibrary.org/obo/GAZ_00387120 -->

    <owl:NamedIndividual rdf:about="http://purl.obolibrary.org/obo/GAZ_00387120">
        <obo:RO_0001025 rdf:resource="http://purl.obolibrary.org/obo/GAZ_00061974"/>
        <obo:IAO_0000115>A subrange of the Muntii Persani.</obo:IAO_0000115>
        <oboInOwl:hasOBONamespace>GAZ</oboInOwl:hasOBONamespace>
        <oboInOwl:id>GAZ:00387120</oboInOwl:id>
        <rdfs:label>Persanii de Sud</rdfs:label>
    </owl:NamedIndividual>
    


    <!-- http://purl.obolibrary.org/obo/GAZ_00387121 -->

    <owl:NamedIndividual rdf:about="http://purl.obolibrary.org/obo/GAZ_00387121">
        <obo:RO_0001025 rdf:resource="http://purl.obolibrary.org/obo/GAZ_00061974"/>
        <obo:IAO_0000115>A subrange of the Muntii Persani.</obo:IAO_0000115>
        <oboInOwl:hasOBONamespace>GAZ</oboInOwl:hasOBONamespace>
        <oboInOwl:id>GAZ:00387121</oboInOwl:id>
        <rdfs:label>Persanii Centrali</rdfs:label>
    </owl:NamedIndividual>
    


    <!-- http://purl.obolibrary.org/obo/GAZ_00387122 -->

    <owl:NamedIndividual rdf:about="http://purl.obolibrary.org/obo/GAZ_00387122">
        <obo:RO_0001025 rdf:resource="http://purl.obolibrary.org/obo/GAZ_00061974"/>
        <obo:IAO_0000115>A subrange of the Muntii Persani.</obo:IAO_0000115>
        <oboInOwl:hasOBONamespace>GAZ</oboInOwl:hasOBONamespace>
        <oboInOwl:id>GAZ:00387122</oboInOwl:id>
        <rdfs:label>Persanii de Nord</rdfs:label>
    </owl:NamedIndividual>
    


    <!-- http://purl.obolibrary.org/obo/GAZ_00387123 -->

    <owl:NamedIndividual rdf:about="http://purl.obolibrary.org/obo/GAZ_00387123">
        <rdf:type rdf:resource="http://purl.obolibrary.org/obo/ENVO_00000100"/>
        <obo:RO_0001025 rdf:resource="http://purl.obolibrary.org/obo/GAZ_00061974"/>
        <obo:IAO_0000115>A gorge.</obo:IAO_0000115>
        <oboInOwl:hasOBONamespace>GAZ</oboInOwl:hasOBONamespace>
        <oboInOwl:id>GAZ:00387123</oboInOwl:id>
        <rdfs:label>Cheile Varghisului</rdfs:label>
    </owl:NamedIndividual>
    


    <!-- http://purl.obolibrary.org/obo/GAZ_00387124 -->

    <owl:NamedIndividual rdf:about="http://purl.obolibrary.org/obo/GAZ_00387124">
        <rdf:type rdf:resource="http://purl.obolibrary.org/obo/ENVO_00000100"/>
        <obo:RO_0001025 rdf:resource="http://purl.obolibrary.org/obo/GAZ_00062025"/>
        <obo:IAO_0000115>A gorge.</obo:IAO_0000115>
        <oboInOwl:hasOBONamespace>GAZ</oboInOwl:hasOBONamespace>
        <oboInOwl:id>GAZ:00387124</oboInOwl:id>
        <rdfs:label>Cheile Valisoarei</rdfs:label>
    </owl:NamedIndividual>
    


    <!-- http://purl.obolibrary.org/obo/GAZ_00387127 -->

    <owl:NamedIndividual rdf:about="http://purl.obolibrary.org/obo/GAZ_00387127">
        <obo:IAO_0000115>A lake.</obo:IAO_0000115>
        <oboInOwl:hasOBONamespace>GAZ</oboInOwl:hasOBONamespace>
        <oboInOwl:id>GAZ:00387127</oboInOwl:id>
        <rdfs:label>Lacul Dobroesti</rdfs:label>
    </owl:NamedIndividual>
    


    <!-- http://purl.obolibrary.org/obo/GAZ_00387128 -->

    <owl:NamedIndividual rdf:about="http://purl.obolibrary.org/obo/GAZ_00387128">
        <obo:IAO_0000115>A reservoir.</obo:IAO_0000115>
        <oboInOwl:hasOBONamespace>GAZ</oboInOwl:hasOBONamespace>
        <oboInOwl:id>GAZ:00387128</oboInOwl:id>
        <rdfs:label>Lacul Rediu</rdfs:label>
    </owl:NamedIndividual>
    


    <!-- http://purl.obolibrary.org/obo/GAZ_00387129 -->

    <owl:NamedIndividual rdf:about="http://purl.obolibrary.org/obo/GAZ_00387129">
        <obo:IAO_0000115>A reservoir.</obo:IAO_0000115>
        <oboInOwl:hasOBONamespace>GAZ</oboInOwl:hasOBONamespace>
        <oboInOwl:id>GAZ:00387129</oboInOwl:id>
        <rdfs:label>Barajul Salcia</rdfs:label>
    </owl:NamedIndividual>
    


    <!-- http://purl.obolibrary.org/obo/GAZ_00387135 -->

    <owl:NamedIndividual rdf:about="http://purl.obolibrary.org/obo/GAZ_00387135">
        <obo:IAO_0000115>A reservoir.</obo:IAO_0000115>
        <oboInOwl:hasOBONamespace>GAZ</oboInOwl:hasOBONamespace>
        <oboInOwl:id>GAZ:00387135</oboInOwl:id>
        <rdfs:label>Barajul Silagiu</rdfs:label>
    </owl:NamedIndividual>
    


    <!-- http://purl.obolibrary.org/obo/GAZ_00387136 -->

    <owl:NamedIndividual rdf:about="http://purl.obolibrary.org/obo/GAZ_00387136">
        <obo:RO_0001025 rdf:resource="http://purl.obolibrary.org/obo/GAZ_00387146"/>
        <obo:IAO_0000115>A reservoir.</obo:IAO_0000115>
        <oboInOwl:hasOBONamespace>GAZ</oboInOwl:hasOBONamespace>
        <oboInOwl:id>GAZ:00387136</oboInOwl:id>
        <rdfs:label>Lacul de acumulare Stramtori</rdfs:label>
    </owl:NamedIndividual>
    


    <!-- http://purl.obolibrary.org/obo/GAZ_00387137 -->

    <owl:NamedIndividual rdf:about="http://purl.obolibrary.org/obo/GAZ_00387137">
        <oboInOwl:hasOBONamespace>GAZ</oboInOwl:hasOBONamespace>
        <oboInOwl:id>GAZ:00387137</oboInOwl:id>
        <rdfs:label>Valea Slipului</rdfs:label>
    </owl:NamedIndividual>
    


    <!-- http://purl.obolibrary.org/obo/GAZ_00387138 -->

    <owl:NamedIndividual rdf:about="http://purl.obolibrary.org/obo/GAZ_00387138">
        <oboInOwl:hasOBONamespace>GAZ</oboInOwl:hasOBONamespace>
        <oboInOwl:id>GAZ:00387138</oboInOwl:id>
        <rdfs:label>Valea Crisului</rdfs:label>
    </owl:NamedIndividual>
    


    <!-- http://purl.obolibrary.org/obo/GAZ_00387139 -->

    <owl:NamedIndividual rdf:about="http://purl.obolibrary.org/obo/GAZ_00387139">
        <oboInOwl:hasOBONamespace>GAZ</oboInOwl:hasOBONamespace>
        <oboInOwl:id>GAZ:00387139</oboInOwl:id>
        <rdfs:label>Frasinet</rdfs:label>
    </owl:NamedIndividual>
    


    <!-- http://purl.obolibrary.org/obo/GAZ_00387140 -->

    <owl:NamedIndividual rdf:about="http://purl.obolibrary.org/obo/GAZ_00387140">
        <oboInOwl:hasOBONamespace>GAZ</oboInOwl:hasOBONamespace>
        <oboInOwl:id>GAZ:00387140</oboInOwl:id>
        <rdfs:label>Valea Limpede</rdfs:label>
    </owl:NamedIndividual>
    


    <!-- http://purl.obolibrary.org/obo/GAZ_00387141 -->

    <owl:NamedIndividual rdf:about="http://purl.obolibrary.org/obo/GAZ_00387141">
        <oboInOwl:hasOBONamespace>GAZ</oboInOwl:hasOBONamespace>
        <oboInOwl:id>GAZ:00387141</oboInOwl:id>
        <rdfs:label>Valea Tulbure</rdfs:label>
    </owl:NamedIndividual>
    


    <!-- http://purl.obolibrary.org/obo/GAZ_00387142 -->

    <owl:NamedIndividual rdf:about="http://purl.obolibrary.org/obo/GAZ_00387142">
        <oboInOwl:hasOBONamespace>GAZ</oboInOwl:hasOBONamespace>
        <oboInOwl:id>GAZ:00387142</oboInOwl:id>
        <rdfs:label>Borcutul</rdfs:label>
    </owl:NamedIndividual>
    


    <!-- http://purl.obolibrary.org/obo/GAZ_00387143 -->

    <owl:NamedIndividual rdf:about="http://purl.obolibrary.org/obo/GAZ_00387143">
        <oboInOwl:hasOBONamespace>GAZ</oboInOwl:hasOBONamespace>
        <oboInOwl:id>GAZ:00387143</oboInOwl:id>
        <rdfs:label>Chiuzbaia</rdfs:label>
    </owl:NamedIndividual>
    


    <!-- http://purl.obolibrary.org/obo/GAZ_00387144 -->

    <owl:NamedIndividual rdf:about="http://purl.obolibrary.org/obo/GAZ_00387144">
        <oboInOwl:hasOBONamespace>GAZ</oboInOwl:hasOBONamespace>
        <oboInOwl:id>GAZ:00387144</oboInOwl:id>
        <rdfs:label>Valea Morii</rdfs:label>
    </owl:NamedIndividual>
    


    <!-- http://purl.obolibrary.org/obo/GAZ_00387145 -->

    <owl:NamedIndividual rdf:about="http://purl.obolibrary.org/obo/GAZ_00387145">
        <oboInOwl:hasOBONamespace>GAZ</oboInOwl:hasOBONamespace>
        <oboInOwl:id>GAZ:00387145</oboInOwl:id>
        <rdfs:label>Valea Gordon</rdfs:label>
    </owl:NamedIndividual>
    


    <!-- http://purl.obolibrary.org/obo/GAZ_00387146 -->

    <owl:NamedIndividual rdf:about="http://purl.obolibrary.org/obo/GAZ_00387146">
        <obo:IAO_0000115>A river.</obo:IAO_0000115>
        <oboInOwl:hasOBONamespace>GAZ</oboInOwl:hasOBONamespace>
        <oboInOwl:id>GAZ:00387146</oboInOwl:id>
        <rdfs:label>Firiza</rdfs:label>
    </owl:NamedIndividual>
    


    <!-- http://purl.obolibrary.org/obo/GAZ_00387147 -->

    <owl:NamedIndividual rdf:about="http://purl.obolibrary.org/obo/GAZ_00387147">
        <oboInOwl:hasOBONamespace>GAZ</oboInOwl:hasOBONamespace>
        <oboInOwl:id>GAZ:00387147</oboInOwl:id>
        <rdfs:label>Usturoiu</rdfs:label>
    </owl:NamedIndividual>
    


    <!-- http://purl.obolibrary.org/obo/GAZ_00387148 -->

    <owl:NamedIndividual rdf:about="http://purl.obolibrary.org/obo/GAZ_00387148">
        <oboInOwl:hasOBONamespace>GAZ</oboInOwl:hasOBONamespace>
        <oboInOwl:id>GAZ:00387148</oboInOwl:id>
        <rdfs:label>Valea Borcutului</rdfs:label>
    </owl:NamedIndividual>
    


    <!-- http://purl.obolibrary.org/obo/GAZ_00387173 -->

    <owl:NamedIndividual rdf:about="http://purl.obolibrary.org/obo/GAZ_00387173">
        <obo:IAO_0000115>A reservoir.</obo:IAO_0000115>
        <oboInOwl:hasOBONamespace>GAZ</oboInOwl:hasOBONamespace>
        <oboInOwl:id>GAZ:00387173</oboInOwl:id>
        <rdfs:label>Barajul Sulita</rdfs:label>
    </owl:NamedIndividual>
    


    <!-- http://purl.obolibrary.org/obo/GAZ_00387174 -->

    <owl:NamedIndividual rdf:about="http://purl.obolibrary.org/obo/GAZ_00387174">
        <obo:IAO_0000115>A reservoir.</obo:IAO_0000115>
        <oboInOwl:hasOBONamespace>GAZ</oboInOwl:hasOBONamespace>
        <oboInOwl:id>GAZ:00387174</oboInOwl:id>
        <rdfs:label>Barajul Turnu</rdfs:label>
    </owl:NamedIndividual>
    


    <!-- http://purl.obolibrary.org/obo/GAZ_00387177 -->

    <owl:NamedIndividual rdf:about="http://purl.obolibrary.org/obo/GAZ_00387177">
        <obo:RO_0001025 rdf:resource="http://purl.obolibrary.org/obo/GAZ_00062006"/>
        <obo:IAO_0000115>A cave.</obo:IAO_0000115>
        <oboInOwl:hasOBONamespace>GAZ</oboInOwl:hasOBONamespace>
        <oboInOwl:id>GAZ:00387177</oboInOwl:id>
        <rdfs:label>Pestera Zeicului</rdfs:label>
    </owl:NamedIndividual>
    


    <!-- http://purl.obolibrary.org/obo/GAZ_00387178 -->

    <owl:NamedIndividual rdf:about="http://purl.obolibrary.org/obo/GAZ_00387178">
        <obo:RO_0001025 rdf:resource="http://purl.obolibrary.org/obo/GAZ_00062004"/>
        <obo:IAO_0000115>A cave.</obo:IAO_0000115>
        <oboInOwl:hasOBONamespace>GAZ</oboInOwl:hasOBONamespace>
        <oboInOwl:id>GAZ:00387178</oboInOwl:id>
        <rdfs:label>Pestera cu Corali</rdfs:label>
    </owl:NamedIndividual>
    


    <!-- http://purl.obolibrary.org/obo/GAZ_00387179 -->

    <owl:NamedIndividual rdf:about="http://purl.obolibrary.org/obo/GAZ_00387179">
        <obo:IAO_0000115>A reservoir.</obo:IAO_0000115>
        <oboInOwl:hasOBONamespace>GAZ</oboInOwl:hasOBONamespace>
        <oboInOwl:id>GAZ:00387179</oboInOwl:id>
        <rdfs:label>Barajul Zetea</rdfs:label>
    </owl:NamedIndividual>
    


    <!-- http://purl.obolibrary.org/obo/GAZ_00387180 -->

    <owl:NamedIndividual rdf:about="http://purl.obolibrary.org/obo/GAZ_00387180">
        <obo:RO_0001025 rdf:resource="http://purl.obolibrary.org/obo/GAZ_00061913"/>
        <obo:IAO_0000115>A natural lake.</obo:IAO_0000115>
        <oboInOwl:hasOBONamespace>GAZ</oboInOwl:hasOBONamespace>
        <oboInOwl:id>GAZ:00387180</oboInOwl:id>
        <rdfs:label>Lacul Cuiejdel</rdfs:label>
    </owl:NamedIndividual>
    


    <!-- http://purl.obolibrary.org/obo/GAZ_00387181 -->

    <owl:NamedIndividual rdf:about="http://purl.obolibrary.org/obo/GAZ_00387181">
        <obo:IAO_0000115>A reservoir.</obo:IAO_0000115>
        <oboInOwl:hasOBONamespace>GAZ</oboInOwl:hasOBONamespace>
        <oboInOwl:id>GAZ:00387181</oboInOwl:id>
        <rdfs:label>Lacul Ciurbesti</rdfs:label>
    </owl:NamedIndividual>
    


    <!-- http://purl.obolibrary.org/obo/GAZ_00387183 -->

    <owl:NamedIndividual rdf:about="http://purl.obolibrary.org/obo/GAZ_00387183">
        <obo:IAO_0000115>A reservoir.</obo:IAO_0000115>
        <oboInOwl:hasOBONamespace>GAZ</oboInOwl:hasOBONamespace>
        <oboInOwl:id>GAZ:00387183</oboInOwl:id>
        <rdfs:label>Lacul Ezareni</rdfs:label>
    </owl:NamedIndividual>
    


    <!-- http://purl.obolibrary.org/obo/GAZ_00387186 -->

    <owl:NamedIndividual rdf:about="http://purl.obolibrary.org/obo/GAZ_00387186">
        <obo:RO_0001025 rdf:resource="http://purl.obolibrary.org/obo/GAZ_00061983"/>
        <obo:IAO_0000115>A reservoir.</obo:IAO_0000115>
        <oboInOwl:hasOBONamespace>GAZ</oboInOwl:hasOBONamespace>
        <oboInOwl:id>GAZ:00387186</oboInOwl:id>
        <rdfs:label>Lacul Bolboci</rdfs:label>
    </owl:NamedIndividual>
    


    <!-- http://purl.obolibrary.org/obo/GAZ_00387187 -->

    <owl:NamedIndividual rdf:about="http://purl.obolibrary.org/obo/GAZ_00387187">
        <obo:IAO_0000115>A reservoir. Impounded by Barajul Somesul Cald.</obo:IAO_0000115>
        <oboInOwl:hasOBONamespace>GAZ</oboInOwl:hasOBONamespace>
        <oboInOwl:id>GAZ:00387187</oboInOwl:id>
        <rdfs:label>Lacul Somesul Cald</rdfs:label>
    </owl:NamedIndividual>
    


    <!-- http://purl.obolibrary.org/obo/GAZ_00387188 -->

    <owl:NamedIndividual rdf:about="http://purl.obolibrary.org/obo/GAZ_00387188">
        <obo:IAO_0000115>A dam. Impounding Lacul Somesul Cald. Constructed 1983.</obo:IAO_0000115>
        <oboInOwl:hasOBONamespace>GAZ</oboInOwl:hasOBONamespace>
        <oboInOwl:id>GAZ:00387188</oboInOwl:id>
        <rdfs:label>Barajul Somesul Cald</rdfs:label>
    </owl:NamedIndividual>
    


    <!-- http://purl.obolibrary.org/obo/GAZ_00387203 -->

    <owl:NamedIndividual rdf:about="http://purl.obolibrary.org/obo/GAZ_00387203">
        <obo:IAO_0000115>A reservoir.</obo:IAO_0000115>
        <oboInOwl:hasOBONamespace>GAZ</oboInOwl:hasOBONamespace>
        <oboInOwl:id>GAZ:00387203</oboInOwl:id>
        <rdfs:label>Lacul de acumulare Vida</rdfs:label>
    </owl:NamedIndividual>
    


    <!-- http://purl.obolibrary.org/obo/GAZ_00387204 -->

    <owl:NamedIndividual rdf:about="http://purl.obolibrary.org/obo/GAZ_00387204">
        <obo:RO_0001025 rdf:resource="http://purl.obolibrary.org/obo/GAZ_00061983"/>
        <obo:IAO_0000115>A lake.</obo:IAO_0000115>
        <oboInOwl:hasOBONamespace>GAZ</oboInOwl:hasOBONamespace>
        <oboInOwl:id>GAZ:00387204</oboInOwl:id>
        <rdfs:label>Lacul Tiganesti</rdfs:label>
    </owl:NamedIndividual>
    


    <!-- http://purl.obolibrary.org/obo/GAZ_00387212 -->

    <owl:NamedIndividual rdf:about="http://purl.obolibrary.org/obo/GAZ_00387212">
        <obo:RO_0001025 rdf:resource="http://purl.obolibrary.org/obo/GAZ_00042222"/>
        <obo:IAO_0000115>An island.</obo:IAO_0000115>
        <oboInOwl:hasOBONamespace>GAZ</oboInOwl:hasOBONamespace>
        <oboInOwl:id>GAZ:00387212</oboInOwl:id>
        <rdfs:label>Insula Bisericuta</rdfs:label>
    </owl:NamedIndividual>
    


    <!-- http://purl.obolibrary.org/obo/GAZ_00387213 -->

    <owl:NamedIndividual rdf:about="http://purl.obolibrary.org/obo/GAZ_00387213">
        <obo:RO_0001025 rdf:resource="http://purl.obolibrary.org/obo/GAZ_00360990"/>
        <obo:IAO_0000115>An island.</obo:IAO_0000115>
        <oboInOwl:hasOBONamespace>GAZ</oboInOwl:hasOBONamespace>
        <oboInOwl:id>GAZ:00387213</oboInOwl:id>
        <rdfs:label>Insula Maican</rdfs:label>
    </owl:NamedIndividual>
    


    <!-- http://purl.obolibrary.org/obo/GAZ_00387217 -->

    <owl:NamedIndividual rdf:about="http://purl.obolibrary.org/obo/GAZ_00387217">
        <obo:RO_0001025 rdf:resource="http://purl.obolibrary.org/obo/GAZ_00061981"/>
        <obo:IAO_0000115>A karst cave.</obo:IAO_0000115>
        <oboInOwl:hasOBONamespace>GAZ</oboInOwl:hasOBONamespace>
        <oboInOwl:id>GAZ:00387217</oboInOwl:id>
        <rdfs:label>Pestera Baia lui Schneider</rdfs:label>
    </owl:NamedIndividual>
    


    <!-- http://purl.obolibrary.org/obo/GAZ_00387218 -->

    <owl:NamedIndividual rdf:about="http://purl.obolibrary.org/obo/GAZ_00387218">
        <obo:RO_0001025 rdf:resource="http://purl.obolibrary.org/obo/GAZ_00062038"/>
        <obo:IAO_0000115>A spring.</obo:IAO_0000115>
        <oboInOwl:hasOBONamespace>GAZ</oboInOwl:hasOBONamespace>
        <oboInOwl:id>GAZ:00387218</oboInOwl:id>
        <rdfs:label>Izbucul Bigar</rdfs:label>
    </owl:NamedIndividual>
    


    <!-- http://purl.obolibrary.org/obo/GAZ_00387220 -->

    <owl:NamedIndividual rdf:about="http://purl.obolibrary.org/obo/GAZ_00387220">
        <obo:RO_0001025 rdf:resource="http://purl.obolibrary.org/obo/GAZ_00062011"/>
        <obo:IAO_0000115>A karst cave.</obo:IAO_0000115>
        <oboInOwl:hasOBONamespace>GAZ</oboInOwl:hasOBONamespace>
        <oboInOwl:id>GAZ:00387220</oboInOwl:id>
        <rdfs:label>Pestera Batranului</rdfs:label>
    </owl:NamedIndividual>
    


    <!-- http://purl.obolibrary.org/obo/GAZ_00387221 -->

    <owl:NamedIndividual rdf:about="http://purl.obolibrary.org/obo/GAZ_00387221">
        <obo:RO_0001025 rdf:resource="http://purl.obolibrary.org/obo/GAZ_00061705"/>
        <obo:IAO_0000115>A cave complex.</obo:IAO_0000115>
        <oboInOwl:hasOBONamespace>GAZ</oboInOwl:hasOBONamespace>
        <oboInOwl:id>GAZ:00387221</oboInOwl:id>
        <rdfs:label>Cetatile Ponorului</rdfs:label>
    </owl:NamedIndividual>
    


    <!-- http://purl.obolibrary.org/obo/GAZ_00387222 -->

    <owl:NamedIndividual rdf:about="http://purl.obolibrary.org/obo/GAZ_00387222">
        <obo:RO_0001025 rdf:resource="http://purl.obolibrary.org/obo/GAZ_00062025"/>
        <obo:RO_0001025 rdf:resource="http://purl.obolibrary.org/obo/GAZ_00387053"/>
        <obo:IAO_0000115>A cave. A paleontological site.</obo:IAO_0000115>
        <oboInOwl:hasOBONamespace>GAZ</oboInOwl:hasOBONamespace>
        <oboInOwl:id>GAZ:00387222</oboInOwl:id>
        <rdfs:label>Pestera Huda lui Papara</rdfs:label>
    </owl:NamedIndividual>
    


    <!-- http://purl.obolibrary.org/obo/GAZ_00387223 -->

    <owl:NamedIndividual rdf:about="http://purl.obolibrary.org/obo/GAZ_00387223">
        <obo:RO_0001025 rdf:resource="http://purl.obolibrary.org/obo/GAZ_00062020"/>
        <obo:IAO_0000115>A protected area.</obo:IAO_0000115>
        <oboInOwl:hasOBONamespace>GAZ</oboInOwl:hasOBONamespace>
        <oboInOwl:id>GAZ:00387223</oboInOwl:id>
        <rdfs:label>Rezervatia naturala Padis</rdfs:label>
    </owl:NamedIndividual>
    


    <!-- http://purl.obolibrary.org/obo/GAZ_00387224 -->

    <owl:NamedIndividual rdf:about="http://purl.obolibrary.org/obo/GAZ_00387224">
        <obo:RO_0001025 rdf:resource="http://purl.obolibrary.org/obo/GAZ_00387223"/>
        <obo:IAO_0000115>A karst cave.</obo:IAO_0000115>
        <oboInOwl:hasOBONamespace>GAZ</oboInOwl:hasOBONamespace>
        <oboInOwl:id>GAZ:00387224</oboInOwl:id>
        <rdfs:label>Pestera de la Caput</rdfs:label>
    </owl:NamedIndividual>
    


    <!-- http://purl.obolibrary.org/obo/GAZ_00387225 -->

    <owl:NamedIndividual rdf:about="http://purl.obolibrary.org/obo/GAZ_00387225">
        <obo:RO_0001025 rdf:resource="http://purl.obolibrary.org/obo/GAZ_00387223"/>
        <obo:IAO_0000115>A karst cave.</obo:IAO_0000115>
        <oboInOwl:hasOBONamespace>GAZ</oboInOwl:hasOBONamespace>
        <oboInOwl:id>GAZ:00387225</oboInOwl:id>
        <rdfs:label>Pestera V5</rdfs:label>
    </owl:NamedIndividual>
    


    <!-- http://purl.obolibrary.org/obo/GAZ_00387226 -->

    <owl:NamedIndividual rdf:about="http://purl.obolibrary.org/obo/GAZ_00387226">
        <obo:RO_0001025 rdf:resource="http://purl.obolibrary.org/obo/GAZ_00061705"/>
        <obo:IAO_0000115>A karst cave.</obo:IAO_0000115>
        <oboInOwl:hasOBONamespace>GAZ</oboInOwl:hasOBONamespace>
        <oboInOwl:id>GAZ:00387226</oboInOwl:id>
        <rdfs:label>Pestera Coliboaia</rdfs:label>
    </owl:NamedIndividual>
    


    <!-- http://purl.obolibrary.org/obo/GAZ_00387227 -->

    <owl:NamedIndividual rdf:about="http://purl.obolibrary.org/obo/GAZ_00387227">
        <obo:RO_0001025 rdf:resource="http://purl.obolibrary.org/obo/GAZ_00387223"/>
        <obo:IAO_0000115>A karst cave.</obo:IAO_0000115>
        <oboInOwl:hasOBONamespace>GAZ</oboInOwl:hasOBONamespace>
        <oboInOwl:id>GAZ:00387227</oboInOwl:id>
        <rdfs:label>Pestera de la Zapodie</rdfs:label>
    </owl:NamedIndividual>
    


    <!-- http://purl.obolibrary.org/obo/GAZ_00387228 -->

    <owl:NamedIndividual rdf:about="http://purl.obolibrary.org/obo/GAZ_00387228">
        <obo:RO_0001025 rdf:resource="http://purl.obolibrary.org/obo/GAZ_00062025"/>
        <obo:IAO_0000115>A karst cave.</obo:IAO_0000115>
        <oboInOwl:hasOBONamespace>GAZ</oboInOwl:hasOBONamespace>
        <oboInOwl:id>GAZ:00387228</oboInOwl:id>
        <rdfs:label>Pestera Calului</rdfs:label>
    </owl:NamedIndividual>
    


    <!-- http://purl.obolibrary.org/obo/GAZ_00387229 -->

    <owl:NamedIndividual rdf:about="http://purl.obolibrary.org/obo/GAZ_00387229">
        <obo:RO_0001025 rdf:resource="http://purl.obolibrary.org/obo/GAZ_00062027"/>
        <obo:IAO_0000115>A karst cave.</obo:IAO_0000115>
        <oboInOwl:hasOBONamespace>GAZ</oboInOwl:hasOBONamespace>
        <oboInOwl:id>GAZ:00387229</oboInOwl:id>
        <rdfs:label>Pestera din Cioaca Birtului</rdfs:label>
    </owl:NamedIndividual>
    


    <!-- http://purl.obolibrary.org/obo/GAZ_00387230 -->

    <owl:NamedIndividual rdf:about="http://purl.obolibrary.org/obo/GAZ_00387230">
        <obo:RO_0001025 rdf:resource="http://purl.obolibrary.org/obo/GAZ_00061974"/>
        <obo:IAO_0000115>A protected area.</obo:IAO_0000115>
        <oboInOwl:hasOBONamespace>GAZ</oboInOwl:hasOBONamespace>
        <oboInOwl:id>GAZ:00387230</oboInOwl:id>
        <rdfs:label>Rezervatia naturala Pestera Comana</rdfs:label>
    </owl:NamedIndividual>
    


    <!-- http://purl.obolibrary.org/obo/GAZ_00387231 -->

    <owl:NamedIndividual rdf:about="http://purl.obolibrary.org/obo/GAZ_00387231">
        <obo:RO_0001025 rdf:resource="http://purl.obolibrary.org/obo/GAZ_00387230"/>
        <obo:IAO_0000115>A karst cave.</obo:IAO_0000115>
        <oboInOwl:hasOBONamespace>GAZ</oboInOwl:hasOBONamespace>
        <oboInOwl:id>GAZ:00387231</oboInOwl:id>
        <rdfs:label>Pestera Comana</rdfs:label>
    </owl:NamedIndividual>
    


    <!-- http://purl.obolibrary.org/obo/GAZ_00387232 -->

    <owl:NamedIndividual rdf:about="http://purl.obolibrary.org/obo/GAZ_00387232">
        <obo:RO_0001025 rdf:resource="http://purl.obolibrary.org/obo/GAZ_00061981"/>
        <obo:IAO_0000115>A karst cave.</obo:IAO_0000115>
        <oboInOwl:hasOBONamespace>GAZ</oboInOwl:hasOBONamespace>
        <oboInOwl:id>GAZ:00387232</oboInOwl:id>
        <rdfs:label>Pestera Cuciulat</rdfs:label>
    </owl:NamedIndividual>
    


    <!-- http://purl.obolibrary.org/obo/GAZ_00387233 -->

    <owl:NamedIndividual rdf:about="http://purl.obolibrary.org/obo/GAZ_00387233">
        <obo:RO_0001025 rdf:resource="http://purl.obolibrary.org/obo/GAZ_00387018"/>
        <obo:IAO_0000115>A karst cave.</obo:IAO_0000115>
        <oboInOwl:hasOBONamespace>GAZ</oboInOwl:hasOBONamespace>
        <oboInOwl:id>GAZ:00387233</oboInOwl:id>
        <rdfs:label>Pestera Dambovicioara</rdfs:label>
    </owl:NamedIndividual>
    


    <!-- http://purl.obolibrary.org/obo/GAZ_00387234 -->

    <owl:NamedIndividual rdf:about="http://purl.obolibrary.org/obo/GAZ_00387234">
        <obo:RO_0001025 rdf:resource="http://purl.obolibrary.org/obo/GAZ_00062020"/>
        <obo:IAO_0000115>A cave.</obo:IAO_0000115>
        <oboInOwl:hasOBONamespace>GAZ</oboInOwl:hasOBONamespace>
        <oboInOwl:id>GAZ:00387234</oboInOwl:id>
        <rdfs:label>Pestera Ghetarul de la Focul Viu</rdfs:label>
    </owl:NamedIndividual>
    


    <!-- http://purl.obolibrary.org/obo/GAZ_00387235 -->

    <owl:NamedIndividual rdf:about="http://purl.obolibrary.org/obo/GAZ_00387235">
        <obo:RO_0001025 rdf:resource="http://purl.obolibrary.org/obo/GAZ_00062011"/>
        <obo:IAO_0000115>A cave.</obo:IAO_0000115>
        <oboInOwl:hasOBONamespace>GAZ</oboInOwl:hasOBONamespace>
        <oboInOwl:id>GAZ:00387235</oboInOwl:id>
        <rdfs:label>Pestera Galaseni</rdfs:label>
    </owl:NamedIndividual>
    


    <!-- http://purl.obolibrary.org/obo/GAZ_00387237 -->

    <owl:NamedIndividual rdf:about="http://purl.obolibrary.org/obo/GAZ_00387237">
        <obo:RO_0001025 rdf:resource="http://purl.obolibrary.org/obo/GAZ_00387018"/>
        <obo:IAO_0000115>A karst cave.</obo:IAO_0000115>
        <oboInOwl:hasOBONamespace>GAZ</oboInOwl:hasOBONamespace>
        <oboInOwl:id>GAZ:00387237</oboInOwl:id>
        <rdfs:label>Pestera cu apa de la Bulz</rdfs:label>
    </owl:NamedIndividual>
    


    <!-- http://purl.obolibrary.org/obo/GAZ_00387238 -->

    <owl:NamedIndividual rdf:about="http://purl.obolibrary.org/obo/GAZ_00387238">
        <obo:RO_0001025 rdf:resource="http://purl.obolibrary.org/obo/GAZ_00062020"/>
        <obo:IAO_0000115>A karst cave.</obo:IAO_0000115>
        <oboInOwl:hasOBONamespace>GAZ</oboInOwl:hasOBONamespace>
        <oboInOwl:id>GAZ:00387238</oboInOwl:id>
        <rdfs:label>Pestera-aven ghetarul de sub Zgurasti</rdfs:label>
    </owl:NamedIndividual>
    


    <!-- http://purl.obolibrary.org/obo/GAZ_00387239 -->

    <owl:NamedIndividual rdf:about="http://purl.obolibrary.org/obo/GAZ_00387239">
        <obo:RO_0001025 rdf:resource="http://purl.obolibrary.org/obo/GAZ_00062025"/>
        <obo:IAO_0000115>A cave.</obo:IAO_0000115>
        <oboInOwl:hasOBONamespace>GAZ</oboInOwl:hasOBONamespace>
        <oboInOwl:id>GAZ:00387239</oboInOwl:id>
        <rdfs:label>Pestera Dambau</rdfs:label>
    </owl:NamedIndividual>
    


    <!-- http://purl.obolibrary.org/obo/GAZ_00387240 -->

    <owl:NamedIndividual rdf:about="http://purl.obolibrary.org/obo/GAZ_00387240">
        <obo:RO_0001025 rdf:resource="http://purl.obolibrary.org/obo/GAZ_00062025"/>
        <obo:IAO_0000115>A cave.</obo:IAO_0000115>
        <oboInOwl:hasOBONamespace>GAZ</oboInOwl:hasOBONamespace>
        <oboInOwl:id>GAZ:00387240</oboInOwl:id>
        <rdfs:label>Pestera Bisericuta</rdfs:label>
    </owl:NamedIndividual>
    


    <!-- http://purl.obolibrary.org/obo/GAZ_00387241 -->

    <owl:NamedIndividual rdf:about="http://purl.obolibrary.org/obo/GAZ_00387241">
        <obo:RO_0001025 rdf:resource="http://purl.obolibrary.org/obo/GAZ_00062020"/>
        <obo:IAO_0000115>A cave.</obo:IAO_0000115>
        <oboInOwl:hasOBONamespace>GAZ</oboInOwl:hasOBONamespace>
        <oboInOwl:id>GAZ:00387241</oboInOwl:id>
        <rdfs:label>Pestera Pojarul Politei</rdfs:label>
    </owl:NamedIndividual>
    


    <!-- http://purl.obolibrary.org/obo/GAZ_00387242 -->

    <owl:NamedIndividual rdf:about="http://purl.obolibrary.org/obo/GAZ_00387242">
        <obo:RO_0001025 rdf:resource="http://purl.obolibrary.org/obo/GAZ_00062020"/>
        <obo:IAO_0000115>A karst pothole.</obo:IAO_0000115>
        <oboInOwl:hasOBONamespace>GAZ</oboInOwl:hasOBONamespace>
        <oboInOwl:id>GAZ:00387242</oboInOwl:id>
        <rdfs:label>Avenul din Sesuri</rdfs:label>
    </owl:NamedIndividual>
    


    <!-- http://purl.obolibrary.org/obo/GAZ_00387243 -->

    <owl:NamedIndividual rdf:about="http://purl.obolibrary.org/obo/GAZ_00387243">
        <obo:RO_0001025 rdf:resource="http://purl.obolibrary.org/obo/GAZ_00062020"/>
        <obo:IAO_0000115>A cave.</obo:IAO_0000115>
        <oboInOwl:hasOBONamespace>GAZ</oboInOwl:hasOBONamespace>
        <oboInOwl:id>GAZ:00387243</oboInOwl:id>
        <rdfs:label>Pestera Gaura Fetii</rdfs:label>
    </owl:NamedIndividual>
    


    <!-- http://purl.obolibrary.org/obo/GAZ_00387244 -->

    <owl:NamedIndividual rdf:about="http://purl.obolibrary.org/obo/GAZ_00387244">
        <obo:RO_0001025 rdf:resource="http://purl.obolibrary.org/obo/GAZ_00062025"/>
        <obo:IAO_0000115>A pothole.</obo:IAO_0000115>
        <oboInOwl:hasOBONamespace>GAZ</oboInOwl:hasOBONamespace>
        <oboInOwl:id>GAZ:00387244</oboInOwl:id>
        <rdfs:label>Avenul Gemenele</rdfs:label>
    </owl:NamedIndividual>
    


    <!-- http://purl.obolibrary.org/obo/GAZ_00387245 -->

    <owl:NamedIndividual rdf:about="http://purl.obolibrary.org/obo/GAZ_00387245">
        <obo:RO_0001025 rdf:resource="http://purl.obolibrary.org/obo/GAZ_00062020"/>
        <obo:IAO_0000115>A cave. A paleontological site.</obo:IAO_0000115>
        <oboInOwl:hasOBONamespace>GAZ</oboInOwl:hasOBONamespace>
        <oboInOwl:id>GAZ:00387245</oboInOwl:id>
        <rdfs:label>Pestera Ghetarul de la Vartop</rdfs:label>
    </owl:NamedIndividual>
    


    <!-- http://purl.obolibrary.org/obo/GAZ_00387247 -->

    <owl:NamedIndividual rdf:about="http://purl.obolibrary.org/obo/GAZ_00387247">
        <obo:RO_0001025 rdf:resource="http://purl.obolibrary.org/obo/GAZ_00062020"/>
        <obo:IAO_0000115>A cave.</obo:IAO_0000115>
        <oboInOwl:hasOBONamespace>GAZ</oboInOwl:hasOBONamespace>
        <oboInOwl:id>GAZ:00387247</oboInOwl:id>
        <rdfs:label>Pestera Poarta lui Ionele</rdfs:label>
    </owl:NamedIndividual>
    


    <!-- http://purl.obolibrary.org/obo/GAZ_00387248 -->

    <owl:NamedIndividual rdf:about="http://purl.obolibrary.org/obo/GAZ_00387248">
        <obo:RO_0001025 rdf:resource="http://purl.obolibrary.org/obo/GAZ_00062020"/>
        <obo:IAO_0000115>A cave.</obo:IAO_0000115>
        <oboInOwl:hasOBONamespace>GAZ</oboInOwl:hasOBONamespace>
        <oboInOwl:id>GAZ:00387248</oboInOwl:id>
        <rdfs:label>Pestera Hodobana</rdfs:label>
    </owl:NamedIndividual>
    


    <!-- http://purl.obolibrary.org/obo/GAZ_00387249 -->

    <owl:NamedIndividual rdf:about="http://purl.obolibrary.org/obo/GAZ_00387249">
        <obo:RO_0001025 rdf:resource="http://purl.obolibrary.org/obo/GAZ_00062020"/>
        <obo:IAO_0000115>A cave.</obo:IAO_0000115>
        <oboInOwl:hasOBONamespace>GAZ</oboInOwl:hasOBONamespace>
        <oboInOwl:id>GAZ:00387249</oboInOwl:id>
        <rdfs:label>Pestera Corobana lui Gartau</rdfs:label>
    </owl:NamedIndividual>
    


    <!-- http://purl.obolibrary.org/obo/GAZ_00387250 -->

    <owl:NamedIndividual rdf:about="http://purl.obolibrary.org/obo/GAZ_00387250">
        <obo:RO_0001025 rdf:resource="http://purl.obolibrary.org/obo/GAZ_00387253"/>
        <obo:IAO_0000115>A karst cave system.</obo:IAO_0000115>
        <oboInOwl:hasOBONamespace>GAZ</oboInOwl:hasOBONamespace>
        <oboInOwl:id>GAZ:00387250</oboInOwl:id>
        <rdfs:label>Pestera cu apa din Valea Firei</rdfs:label>
    </owl:NamedIndividual>
    


    <!-- http://purl.obolibrary.org/obo/GAZ_00387251 -->

    <owl:NamedIndividual rdf:about="http://purl.obolibrary.org/obo/GAZ_00387251">
        <obo:RO_0001025 rdf:resource="http://purl.obolibrary.org/obo/GAZ_00387250"/>
        <obo:IAO_0000115>A karst cave system.</obo:IAO_0000115>
        <oboInOwl:hasOBONamespace>GAZ</oboInOwl:hasOBONamespace>
        <oboInOwl:id>GAZ:00387251</oboInOwl:id>
        <rdfs:label>Pestera Mare din Valea Firei</rdfs:label>
    </owl:NamedIndividual>
    


    <!-- http://purl.obolibrary.org/obo/GAZ_00387252 -->

    <owl:NamedIndividual rdf:about="http://purl.obolibrary.org/obo/GAZ_00387252">
        <obo:RO_0001025 rdf:resource="http://purl.obolibrary.org/obo/GAZ_00387250"/>
        <obo:IAO_0000115>A karst cave system.</obo:IAO_0000115>
        <oboInOwl:hasOBONamespace>GAZ</oboInOwl:hasOBONamespace>
        <oboInOwl:id>GAZ:00387252</oboInOwl:id>
        <rdfs:label>Avenul din Poienita</rdfs:label>
    </owl:NamedIndividual>
    


    <!-- http://purl.obolibrary.org/obo/GAZ_00387253 -->

    <owl:NamedIndividual rdf:about="http://purl.obolibrary.org/obo/GAZ_00387253">
        <obo:RO_0001025 rdf:resource="http://purl.obolibrary.org/obo/GAZ_00062020"/>
        <obo:IAO_0000115>A karst cave complex.</obo:IAO_0000115>
        <oboInOwl:hasOBONamespace>GAZ</oboInOwl:hasOBONamespace>
        <oboInOwl:id>GAZ:00387253</oboInOwl:id>
        <rdfs:label>Sistemul Humpleu</rdfs:label>
    </owl:NamedIndividual>
    


    <!-- http://purl.obolibrary.org/obo/GAZ_00387254 -->

    <owl:NamedIndividual rdf:about="http://purl.obolibrary.org/obo/GAZ_00387254">
        <obo:RO_0001025 rdf:resource="http://purl.obolibrary.org/obo/GAZ_00062003"/>
        <obo:IAO_0000115>A cave.</obo:IAO_0000115>
        <oboInOwl:hasOBONamespace>GAZ</oboInOwl:hasOBONamespace>
        <oboInOwl:id>GAZ:00387254</oboInOwl:id>
        <rdfs:label>Pestera Bolii</rdfs:label>
    </owl:NamedIndividual>
    


    <!-- http://purl.obolibrary.org/obo/GAZ_00387255 -->

    <owl:NamedIndividual rdf:about="http://purl.obolibrary.org/obo/GAZ_00387255">
        <obo:RO_0001025 rdf:resource="http://purl.obolibrary.org/obo/GAZ_00062020"/>
        <obo:IAO_0000115>A cave.</obo:IAO_0000115>
        <oboInOwl:hasOBONamespace>GAZ</oboInOwl:hasOBONamespace>
        <oboInOwl:id>GAZ:00387255</oboInOwl:id>
        <rdfs:label>Izbucul de la Cotetul Dobrestilor</rdfs:label>
    </owl:NamedIndividual>
    


    <!-- http://purl.obolibrary.org/obo/GAZ_00387256 -->

    <owl:NamedIndividual rdf:about="http://purl.obolibrary.org/obo/GAZ_00387256">
        <obo:RO_0001025 rdf:resource="http://purl.obolibrary.org/obo/GAZ_00062025"/>
        <obo:IAO_0000115>A karst cave.</obo:IAO_0000115>
        <oboInOwl:hasOBONamespace>GAZ</oboInOwl:hasOBONamespace>
        <oboInOwl:id>GAZ:00387256</oboInOwl:id>
        <rdfs:label>Pestera din Dealul Cornului</rdfs:label>
    </owl:NamedIndividual>
    


    <!-- http://purl.obolibrary.org/obo/GAZ_00387257 -->

    <owl:NamedIndividual rdf:about="http://purl.obolibrary.org/obo/GAZ_00387257">
        <obo:RO_0001025 rdf:resource="http://purl.obolibrary.org/obo/GAZ_00062025"/>
        <obo:IAO_0000115>A cave.</obo:IAO_0000115>
        <oboInOwl:hasOBONamespace>GAZ</oboInOwl:hasOBONamespace>
        <oboInOwl:id>GAZ:00387257</oboInOwl:id>
        <rdfs:label>Pestera Dalbina</rdfs:label>
    </owl:NamedIndividual>
    


    <!-- http://purl.obolibrary.org/obo/GAZ_00387258 -->

    <owl:NamedIndividual rdf:about="http://purl.obolibrary.org/obo/GAZ_00387258">
        <obo:RO_0001025 rdf:resource="http://purl.obolibrary.org/obo/GAZ_00062025"/>
        <obo:IAO_0000115>A karst cave.</obo:IAO_0000115>
        <oboInOwl:hasOBONamespace>GAZ</oboInOwl:hasOBONamespace>
        <oboInOwl:id>GAZ:00387258</oboInOwl:id>
        <rdfs:label>Pestera Mica de la Vanatare</rdfs:label>
    </owl:NamedIndividual>
    


    <!-- http://purl.obolibrary.org/obo/GAZ_00387260 -->

    <owl:NamedIndividual rdf:about="http://purl.obolibrary.org/obo/GAZ_00387260">
        <obo:RO_0001025 rdf:resource="http://purl.obolibrary.org/obo/GAZ_00062025"/>
        <obo:IAO_0000115>A pothole.</obo:IAO_0000115>
        <oboInOwl:hasOBONamespace>GAZ</oboInOwl:hasOBONamespace>
        <oboInOwl:id>GAZ:00387260</oboInOwl:id>
        <rdfs:label>Avenul din Piatra Cetii</rdfs:label>
    </owl:NamedIndividual>
    


    <!-- http://purl.obolibrary.org/obo/GAZ_00387261 -->

    <owl:NamedIndividual rdf:about="http://purl.obolibrary.org/obo/GAZ_00387261">
        <obo:RO_0001025 rdf:resource="http://purl.obolibrary.org/obo/GAZ_00061981"/>
        <obo:IAO_0000115>A karst cave.</obo:IAO_0000115>
        <oboInOwl:hasOBONamespace>GAZ</oboInOwl:hasOBONamespace>
        <oboInOwl:id>GAZ:00387261</oboInOwl:id>
        <rdfs:label>Pestera Izvorul Tausoarelor</rdfs:label>
    </owl:NamedIndividual>
    


    <!-- http://purl.obolibrary.org/obo/GAZ_00387262 -->

    <owl:NamedIndividual rdf:about="http://purl.obolibrary.org/obo/GAZ_00387262">
        <obo:RO_0001025 rdf:resource="http://purl.obolibrary.org/obo/GAZ_00061981"/>
        <obo:IAO_0000115>A cave.</obo:IAO_0000115>
        <oboInOwl:hasOBONamespace>GAZ</oboInOwl:hasOBONamespace>
        <oboInOwl:id>GAZ:00387262</oboInOwl:id>
        <rdfs:label>Pestera Izvorul Albastru al Izei</rdfs:label>
    </owl:NamedIndividual>
    


    <!-- http://purl.obolibrary.org/obo/GAZ_00387264 -->

    <owl:NamedIndividual rdf:about="http://purl.obolibrary.org/obo/GAZ_00387264">
        <obo:RO_0001025 rdf:resource="http://purl.obolibrary.org/obo/GAZ_00062011"/>
        <obo:IAO_0000115>A cave.</obo:IAO_0000115>
        <oboInOwl:hasOBONamespace>GAZ</oboInOwl:hasOBONamespace>
        <oboInOwl:id>GAZ:00387264</oboInOwl:id>
        <rdfs:label>Pestera Izbandis</rdfs:label>
    </owl:NamedIndividual>
    


    <!-- http://purl.obolibrary.org/obo/GAZ_00387265 -->

    <owl:NamedIndividual rdf:about="http://purl.obolibrary.org/obo/GAZ_00387265">
        <obo:RO_0001025 rdf:resource="http://purl.obolibrary.org/obo/GAZ_00061981"/>
        <obo:IAO_0000115>A karst cave.</obo:IAO_0000115>
        <oboInOwl:hasOBONamespace>GAZ</oboInOwl:hasOBONamespace>
        <oboInOwl:id>GAZ:00387265</oboInOwl:id>
        <rdfs:label>Pestera Jgheabul lui Zalion</rdfs:label>
    </owl:NamedIndividual>
    


    <!-- http://purl.obolibrary.org/obo/GAZ_00387266 -->

    <owl:NamedIndividual rdf:about="http://purl.obolibrary.org/obo/GAZ_00387266">
        <obo:RO_0001025 rdf:resource="http://purl.obolibrary.org/obo/GAZ_00062011"/>
        <obo:IAO_0000115>A cave.</obo:IAO_0000115>
        <oboInOwl:hasOBONamespace>GAZ</oboInOwl:hasOBONamespace>
        <oboInOwl:id>GAZ:00387266</oboInOwl:id>
        <rdfs:label>Pestera Moanei</rdfs:label>
    </owl:NamedIndividual>
    


    <!-- http://purl.obolibrary.org/obo/GAZ_00387267 -->

    <owl:NamedIndividual rdf:about="http://purl.obolibrary.org/obo/GAZ_00387267">
        <obo:RO_0001025 rdf:resource="http://purl.obolibrary.org/obo/GAZ_00062011"/>
        <obo:IAO_0000115>A cave.</obo:IAO_0000115>
        <oboInOwl:hasOBONamespace>GAZ</oboInOwl:hasOBONamespace>
        <oboInOwl:id>GAZ:00387267</oboInOwl:id>
        <rdfs:label>Pestera Lesiana</rdfs:label>
    </owl:NamedIndividual>
    


    <!-- http://purl.obolibrary.org/obo/GAZ_00387268 -->

    <owl:NamedIndividual rdf:about="http://purl.obolibrary.org/obo/GAZ_00387268">
        <obo:RO_0001025 rdf:resource="http://purl.obolibrary.org/obo/GAZ_00062011"/>
        <obo:IAO_0000115>A cave.</obo:IAO_0000115>
        <oboInOwl:hasOBONamespace>GAZ</oboInOwl:hasOBONamespace>
        <oboInOwl:id>GAZ:00387268</oboInOwl:id>
        <rdfs:label>Pestera cu Apa din Valea Lesului</rdfs:label>
    </owl:NamedIndividual>
    


    <!-- http://purl.obolibrary.org/obo/GAZ_00387271 -->

    <owl:NamedIndividual rdf:about="http://purl.obolibrary.org/obo/GAZ_00387271">
        <obo:RO_0001025 rdf:resource="http://purl.obolibrary.org/obo/GAZ_00061981"/>
        <obo:IAO_0000115>A cave.</obo:IAO_0000115>
        <oboInOwl:hasOBONamespace>GAZ</oboInOwl:hasOBONamespace>
        <oboInOwl:id>GAZ:00387271</oboInOwl:id>
        <rdfs:label>Pestera Maglei</rdfs:label>
    </owl:NamedIndividual>
    


    <!-- http://purl.obolibrary.org/obo/GAZ_00387272 -->

    <owl:NamedIndividual rdf:about="http://purl.obolibrary.org/obo/GAZ_00387272">
        <obo:RO_0001025 rdf:resource="http://purl.obolibrary.org/obo/GAZ_00062011"/>
        <obo:IAO_0000115>A cave.</obo:IAO_0000115>
        <oboInOwl:hasOBONamespace>GAZ</oboInOwl:hasOBONamespace>
        <oboInOwl:id>GAZ:00387272</oboInOwl:id>
        <rdfs:label>Pestera Meziad</rdfs:label>
    </owl:NamedIndividual>
    


    <!-- http://purl.obolibrary.org/obo/GAZ_00387273 -->

    <owl:NamedIndividual rdf:about="http://purl.obolibrary.org/obo/GAZ_00387273">
        <obo:RO_0001025 rdf:resource="http://purl.obolibrary.org/obo/GAZ_00062011"/>
        <obo:IAO_0000115>A cave.</obo:IAO_0000115>
        <oboInOwl:hasOBONamespace>GAZ</oboInOwl:hasOBONamespace>
        <oboInOwl:id>GAZ:00387273</oboInOwl:id>
        <rdfs:label>Pestera Muhuchii</rdfs:label>
    </owl:NamedIndividual>
    


    <!-- http://purl.obolibrary.org/obo/GAZ_00387274 -->

    <owl:NamedIndividual rdf:about="http://purl.obolibrary.org/obo/GAZ_00387274">
        <obo:RO_0001025 rdf:resource="http://purl.obolibrary.org/obo/GAZ_00062011"/>
        <obo:IAO_0000115>A cave.</obo:IAO_0000115>
        <oboInOwl:hasOBONamespace>GAZ</oboInOwl:hasOBONamespace>
        <oboInOwl:id>GAZ:00387274</oboInOwl:id>
        <rdfs:label>Pestera Osoi</rdfs:label>
    </owl:NamedIndividual>
    


    <!-- http://purl.obolibrary.org/obo/GAZ_00387276 -->

    <owl:NamedIndividual rdf:about="http://purl.obolibrary.org/obo/GAZ_00387276">
        <obo:RO_0001025 rdf:resource="http://purl.obolibrary.org/obo/GAZ_00061705"/>
        <obo:IAO_0000115>A mountain basin.</obo:IAO_0000115>
        <oboInOwl:hasOBONamespace>GAZ</oboInOwl:hasOBONamespace>
        <oboInOwl:id>GAZ:00387276</oboInOwl:id>
        <rdfs:label>Poiana Ponor</rdfs:label>
    </owl:NamedIndividual>
    


    <!-- http://purl.obolibrary.org/obo/GAZ_00387277 -->

    <owl:NamedIndividual rdf:about="http://purl.obolibrary.org/obo/GAZ_00387277">
        <obo:RO_0001025 rdf:resource="http://purl.obolibrary.org/obo/GAZ_00062020"/>
        <obo:IAO_0000115>A karst cave.</obo:IAO_0000115>
        <oboInOwl:hasOBONamespace>GAZ</oboInOwl:hasOBONamespace>
        <oboInOwl:id>GAZ:00387277</oboInOwl:id>
        <rdfs:label>Pestera din Peretele Darnini</rdfs:label>
    </owl:NamedIndividual>
    


    <!-- http://purl.obolibrary.org/obo/GAZ_00387278 -->

    <owl:NamedIndividual rdf:about="http://purl.obolibrary.org/obo/GAZ_00387278">
        <obo:RO_0001025 rdf:resource="http://purl.obolibrary.org/obo/GAZ_00062011"/>
        <obo:IAO_0000115>A karst cave.</obo:IAO_0000115>
        <oboInOwl:hasOBONamespace>GAZ</oboInOwl:hasOBONamespace>
        <oboInOwl:id>GAZ:00387278</oboInOwl:id>
        <rdfs:label>Pestera Ciurul Ponor</rdfs:label>
    </owl:NamedIndividual>
    


    <!-- http://purl.obolibrary.org/obo/GAZ_00387285 -->

    <owl:NamedIndividual rdf:about="http://purl.obolibrary.org/obo/GAZ_00387285">
        <obo:RO_0001025 rdf:resource="http://purl.obolibrary.org/obo/GAZ_00062027"/>
        <obo:IAO_0000115>A cave.</obo:IAO_0000115>
        <oboInOwl:hasOBONamespace>GAZ</oboInOwl:hasOBONamespace>
        <oboInOwl:id>GAZ:00387285</oboInOwl:id>
        <rdfs:label>Pestera Piatra Fetii</rdfs:label>
    </owl:NamedIndividual>
    


    <!-- http://purl.obolibrary.org/obo/GAZ_00387286 -->

    <owl:NamedIndividual rdf:about="http://purl.obolibrary.org/obo/GAZ_00387286">
        <obo:RO_0001025 rdf:resource="http://purl.obolibrary.org/obo/GAZ_00062011"/>
        <obo:IAO_0000115>A cave.</obo:IAO_0000115>
        <oboInOwl:hasOBONamespace>GAZ</oboInOwl:hasOBONamespace>
        <oboInOwl:id>GAZ:00387286</oboInOwl:id>
        <rdfs:label>Pestera Pietrarului</rdfs:label>
    </owl:NamedIndividual>
    


    <!-- http://purl.obolibrary.org/obo/GAZ_00387291 -->

    <owl:NamedIndividual rdf:about="http://purl.obolibrary.org/obo/GAZ_00387291">
        <obo:RO_0001025 rdf:resource="http://purl.obolibrary.org/obo/GAZ_00062027"/>
        <obo:IAO_0000115>A cave.</obo:IAO_0000115>
        <oboInOwl:hasOBONamespace>GAZ</oboInOwl:hasOBONamespace>
        <oboInOwl:id>GAZ:00387291</oboInOwl:id>
        <rdfs:label>Pestera Romanesti</rdfs:label>
    </owl:NamedIndividual>
    


    <!-- http://purl.obolibrary.org/obo/GAZ_00387292 -->

    <owl:NamedIndividual rdf:about="http://purl.obolibrary.org/obo/GAZ_00387292">
        <obo:RO_0001025 rdf:resource="http://purl.obolibrary.org/obo/GAZ_00387084"/>
        <obo:IAO_0000115>A cave.</obo:IAO_0000115>
        <oboInOwl:hasOBONamespace>GAZ</oboInOwl:hasOBONamespace>
        <oboInOwl:id>GAZ:00387292</oboInOwl:id>
        <rdfs:label>Pestera Rasnoavei</rdfs:label>
    </owl:NamedIndividual>
    


    <!-- http://purl.obolibrary.org/obo/GAZ_00387294 -->

    <owl:NamedIndividual rdf:about="http://purl.obolibrary.org/obo/GAZ_00387294">
        <obo:RO_0001025 rdf:resource="http://purl.obolibrary.org/obo/GAZ_00062020"/>
        <obo:IAO_0000115>A karst pothole.</obo:IAO_0000115>
        <oboInOwl:hasOBONamespace>GAZ</oboInOwl:hasOBONamespace>
        <oboInOwl:id>GAZ:00387294</oboInOwl:id>
        <rdfs:label>Avenul de la Mununa</rdfs:label>
    </owl:NamedIndividual>
    


    <!-- http://purl.obolibrary.org/obo/GAZ_00387295 -->

    <owl:NamedIndividual rdf:about="http://purl.obolibrary.org/obo/GAZ_00387295">
        <obo:RO_0001025 rdf:resource="http://purl.obolibrary.org/obo/GAZ_00062027"/>
        <obo:IAO_0000115>A cave.</obo:IAO_0000115>
        <oboInOwl:hasOBONamespace>GAZ</oboInOwl:hasOBONamespace>
        <oboInOwl:id>GAZ:00387295</oboInOwl:id>
        <rdfs:label>Pestera din Stanca lui Florian</rdfs:label>
    </owl:NamedIndividual>
    


    <!-- http://purl.obolibrary.org/obo/GAZ_00387297 -->

    <owl:NamedIndividual rdf:about="http://purl.obolibrary.org/obo/GAZ_00387297">
        <rdf:type rdf:resource="http://purl.obolibrary.org/obo/ENVO_00000100"/>
        <obo:RO_0001025 rdf:resource="http://purl.obolibrary.org/obo/GAZ_00062011"/>
        <obo:IAO_0000115>A gorge.</obo:IAO_0000115>
        <oboInOwl:hasOBONamespace>GAZ</oboInOwl:hasOBONamespace>
        <oboInOwl:id>GAZ:00387297</oboInOwl:id>
        <rdfs:label>Defileul Crisului Repede</rdfs:label>
    </owl:NamedIndividual>
    


    <!-- http://purl.obolibrary.org/obo/GAZ_00387298 -->

    <owl:NamedIndividual rdf:about="http://purl.obolibrary.org/obo/GAZ_00387298">
        <obo:RO_0001025 rdf:resource="http://purl.obolibrary.org/obo/GAZ_00387297"/>
        <obo:IAO_0000115>A cave.</obo:IAO_0000115>
        <oboInOwl:hasOBONamespace>GAZ</oboInOwl:hasOBONamespace>
        <oboInOwl:id>GAZ:00387298</oboInOwl:id>
        <rdfs:label>Pestera Unguru Mare</rdfs:label>
    </owl:NamedIndividual>
    


    <!-- http://purl.obolibrary.org/obo/GAZ_00387301 -->

    <owl:NamedIndividual rdf:about="http://purl.obolibrary.org/obo/GAZ_00387301">
        <obo:RO_0001025 rdf:resource="http://purl.obolibrary.org/obo/GAZ_00062011"/>
        <obo:IAO_0000115>A karst cave.</obo:IAO_0000115>
        <oboInOwl:hasOBONamespace>GAZ</oboInOwl:hasOBONamespace>
        <oboInOwl:id>GAZ:00387301</oboInOwl:id>
        <rdfs:label>Pestera Vantului</rdfs:label>
    </owl:NamedIndividual>
    


    <!-- http://purl.obolibrary.org/obo/GAZ_00387302 -->

    <owl:NamedIndividual rdf:about="http://purl.obolibrary.org/obo/GAZ_00387302">
        <obo:RO_0001025 rdf:resource="http://purl.obolibrary.org/obo/GAZ_00061981"/>
        <obo:IAO_0000115>A cave.</obo:IAO_0000115>
        <oboInOwl:hasOBONamespace>GAZ</oboInOwl:hasOBONamespace>
        <oboInOwl:id>GAZ:00387302</oboInOwl:id>
        <rdfs:label>Pestera Grota Zanelor</rdfs:label>
    </owl:NamedIndividual>
    


    <!-- http://purl.obolibrary.org/obo/GAZ_00387303 -->

    <owl:NamedIndividual rdf:about="http://purl.obolibrary.org/obo/GAZ_00387303">
        <obo:IAO_0000115>A cave.</obo:IAO_0000115>
        <oboInOwl:hasOBONamespace>GAZ</oboInOwl:hasOBONamespace>
        <oboInOwl:id>GAZ:00387303</oboInOwl:id>
        <rdfs:label>Pestera Varfurasu</rdfs:label>
    </owl:NamedIndividual>
    


    <!-- http://purl.obolibrary.org/obo/GAZ_00387304 -->

    <owl:NamedIndividual rdf:about="http://purl.obolibrary.org/obo/GAZ_00387304">
        <rdf:type rdf:resource="http://purl.obolibrary.org/obo/ENVO_00000080"/>
        <obo:RO_0001025 rdf:resource="http://purl.obolibrary.org/obo/GAZ_00061705"/>
        <obo:IAO_0000115>A mountain group.</obo:IAO_0000115>
        <oboInOwl:hasOBONamespace>GAZ</oboInOwl:hasOBONamespace>
        <oboInOwl:id>GAZ:00387304</oboInOwl:id>
        <rdfs:label>Masivul Vladeasa</rdfs:label>
    </owl:NamedIndividual>
    


    <!-- http://purl.obolibrary.org/obo/GAZ_00465556 -->

    <owl:NamedIndividual rdf:about="http://purl.obolibrary.org/obo/GAZ_00465556">
        <obo:RO_0001025 rdf:resource="http://purl.obolibrary.org/obo/GAZ_00061716"/>
        <obo:IAO_0000115>A protected area.</obo:IAO_0000115>
        <oboInOwl:hasOBONamespace>GAZ</oboInOwl:hasOBONamespace>
        <oboInOwl:id>GAZ:00465556</oboInOwl:id>
        <rdfs:label>Chranene krajinne oblasti Poodri</rdfs:label>
    </owl:NamedIndividual>
    


    <!-- http://purl.obolibrary.org/obo/GAZ_00465557 -->

    <owl:NamedIndividual rdf:about="http://purl.obolibrary.org/obo/GAZ_00465557">
        <obo:RO_0001025 rdf:resource="http://purl.obolibrary.org/obo/GAZ_00061755"/>
        <obo:IAO_0000115>A protected area that lies in the south-eastern part of the Moravian Silesian and eastern part of Zlin regions, on the border with Slovakia. All its area belongs to the Outer Western Carpathians and comprises most of Moravian-Silesian Beskids Range, large part of the Vsetinske vrchy Range and the Moravian part of the Javorniky Range. In Slovakia, Kysuce Protected Landscape Area borders the area. Established 1973-03-05.</obo:IAO_0000115>
        <oboInOwl:hasOBONamespace>GAZ</oboInOwl:hasOBONamespace>
        <oboInOwl:id>GAZ:00465557</oboInOwl:id>
        <rdfs:label>Chranena krajinna oblast Beskydy</rdfs:label>
    </owl:NamedIndividual>
    


    <!-- http://purl.obolibrary.org/obo/GAZ_00465642 -->

    <owl:NamedIndividual rdf:about="http://purl.obolibrary.org/obo/GAZ_00465642">
        <obo:IAO_0000115>A dam.</obo:IAO_0000115>
        <oboInOwl:hasOBONamespace>GAZ</oboInOwl:hasOBONamespace>
        <oboInOwl:id>GAZ:00465642</oboInOwl:id>
        <rdfs:label>Mohelno prehradni</rdfs:label>
    </owl:NamedIndividual>
    


    <!-- http://purl.obolibrary.org/obo/GAZ_00465649 -->

    <owl:NamedIndividual rdf:about="http://purl.obolibrary.org/obo/GAZ_00465649">
        <obo:IAO_0000115>A dam.</obo:IAO_0000115>
        <oboInOwl:hasOBONamespace>GAZ</oboInOwl:hasOBONamespace>
        <oboInOwl:id>GAZ:00465649</oboInOwl:id>
        <rdfs:label>Mostiste prehradni</rdfs:label>
    </owl:NamedIndividual>
    


    <!-- http://purl.obolibrary.org/obo/GAZ_00465749 -->

    <owl:NamedIndividual rdf:about="http://purl.obolibrary.org/obo/GAZ_00465749">
        <obo:IAO_0000115>A lake.</obo:IAO_0000115>
        <oboInOwl:hasOBONamespace>GAZ</oboInOwl:hasOBONamespace>
        <oboInOwl:id>GAZ:00465749</oboInOwl:id>
        <rdfs:label>Vrbatecky nahon</rdfs:label>
    </owl:NamedIndividual>
    


    <!-- http://purl.obolibrary.org/obo/GAZ_00465750 -->

    <owl:NamedIndividual rdf:about="http://purl.obolibrary.org/obo/GAZ_00465750">
        <obo:IAO_0000115>A lake.</obo:IAO_0000115>
        <oboInOwl:hasOBONamespace>GAZ</oboInOwl:hasOBONamespace>
        <oboInOwl:id>GAZ:00465750</oboInOwl:id>
        <rdfs:label>Mlynsky nahon</rdfs:label>
    </owl:NamedIndividual>
    


    <!-- http://purl.obolibrary.org/obo/GAZ_00465805 -->

    <owl:NamedIndividual rdf:about="http://purl.obolibrary.org/obo/GAZ_00465805">
        <obo:IAO_0000115>A lake.</obo:IAO_0000115>
        <oboInOwl:hasOBONamespace>GAZ</oboInOwl:hasOBONamespace>
        <oboInOwl:id>GAZ:00465805</oboInOwl:id>
        <rdfs:label>Treti voda</rdfs:label>
    </owl:NamedIndividual>
    


    <!-- http://purl.obolibrary.org/obo/GAZ_00465806 -->

    <owl:NamedIndividual rdf:about="http://purl.obolibrary.org/obo/GAZ_00465806">
        <obo:IAO_0000115>A lake.</obo:IAO_0000115>
        <oboInOwl:hasOBONamespace>GAZ</oboInOwl:hasOBONamespace>
        <oboInOwl:id>GAZ:00465806</oboInOwl:id>
        <rdfs:label>Kobylnik</rdfs:label>
    </owl:NamedIndividual>
    


    <!-- http://purl.obolibrary.org/obo/GAZ_00466014 -->

    <owl:NamedIndividual rdf:about="http://purl.obolibrary.org/obo/GAZ_00466014">
        <obo:RO_0001025 rdf:resource="http://purl.obolibrary.org/obo/GAZ_00061695"/>
        <obo:IAO_0000115>A protected area.</obo:IAO_0000115>
        <oboInOwl:hasOBONamespace>GAZ</oboInOwl:hasOBONamespace>
        <oboInOwl:id>GAZ:00466014</oboInOwl:id>
        <rdfs:label>Chranena krajinna oblast Palava</rdfs:label>
    </owl:NamedIndividual>
    


    <!-- http://purl.obolibrary.org/obo/GAZ_00466054 -->

    <owl:NamedIndividual rdf:about="http://purl.obolibrary.org/obo/GAZ_00466054">
        <obo:IAO_0000115>A river.</obo:IAO_0000115>
        <oboInOwl:hasOBONamespace>GAZ</oboInOwl:hasOBONamespace>
        <oboInOwl:id>GAZ:00466054</oboInOwl:id>
        <rdfs:label>Kamenicka</rdfs:label>
    </owl:NamedIndividual>
    


    <!-- http://purl.obolibrary.org/obo/GAZ_00466055 -->

    <owl:NamedIndividual rdf:about="http://purl.obolibrary.org/obo/GAZ_00466055">
        <obo:RO_0001025 rdf:resource="http://purl.obolibrary.org/obo/GAZ_00466054"/>
        <obo:IAO_0000115>A reservoir.</obo:IAO_0000115>
        <oboInOwl:hasOBONamespace>GAZ</oboInOwl:hasOBONamespace>
        <oboInOwl:id>GAZ:00466055</oboInOwl:id>
        <rdfs:label>Vodni nadrz Kamenicka</rdfs:label>
    </owl:NamedIndividual>
    


    <!-- http://purl.obolibrary.org/obo/GAZ_00466056 -->

    <owl:NamedIndividual rdf:about="http://purl.obolibrary.org/obo/GAZ_00466056">
        <obo:RO_0001025 rdf:resource="http://purl.obolibrary.org/obo/GAZ_00466054"/>
        <obo:IAO_0000115>A dam.</obo:IAO_0000115>
        <oboInOwl:hasOBONamespace>GAZ</oboInOwl:hasOBONamespace>
        <oboInOwl:id>GAZ:00466056</oboInOwl:id>
        <rdfs:label>Prehrada Kamenicka</rdfs:label>
    </owl:NamedIndividual>
    


    <!-- http://purl.obolibrary.org/obo/GAZ_00466068 -->

    <owl:NamedIndividual rdf:about="http://purl.obolibrary.org/obo/GAZ_00466068">
        <obo:RO_0001025 rdf:resource="http://purl.obolibrary.org/obo/GAZ_00466069"/>
        <obo:IAO_0000115>A reservoir.</obo:IAO_0000115>
        <oboInOwl:hasOBONamespace>GAZ</oboInOwl:hasOBONamespace>
        <oboInOwl:id>GAZ:00466068</oboInOwl:id>
        <rdfs:label>Vodni nadrz Krimov</rdfs:label>
    </owl:NamedIndividual>
    


    <!-- http://purl.obolibrary.org/obo/GAZ_00466069 -->

    <owl:NamedIndividual rdf:about="http://purl.obolibrary.org/obo/GAZ_00466069">
        <obo:IAO_0000115>A river.</obo:IAO_0000115>
        <oboInOwl:hasOBONamespace>GAZ</oboInOwl:hasOBONamespace>
        <oboInOwl:id>GAZ:00466069</oboInOwl:id>
        <rdfs:label>Krimovsky potok</rdfs:label>
    </owl:NamedIndividual>
    


    <!-- http://purl.obolibrary.org/obo/GAZ_00466193 -->

    <owl:NamedIndividual rdf:about="http://purl.obolibrary.org/obo/GAZ_00466193">
        <obo:IAO_0000115>A dam and reservoir.</obo:IAO_0000115>
        <oboInOwl:hasOBONamespace>GAZ</oboInOwl:hasOBONamespace>
        <oboInOwl:id>GAZ:00466193</oboInOwl:id>
        <rdfs:label>Slusovice Dam</rdfs:label>
    </owl:NamedIndividual>
    


    <!-- http://purl.obolibrary.org/obo/GAZ_00466197 -->

    <owl:NamedIndividual rdf:about="http://purl.obolibrary.org/obo/GAZ_00466197">
        <obo:IAO_0000115>A reservoir.</obo:IAO_0000115>
        <oboInOwl:hasOBONamespace>GAZ</oboInOwl:hasOBONamespace>
        <oboInOwl:id>GAZ:00466197</oboInOwl:id>
        <rdfs:label>Vodni nadrz Bystricka</rdfs:label>
    </owl:NamedIndividual>
    


    <!-- http://purl.obolibrary.org/obo/GAZ_00466217 -->

    <owl:NamedIndividual rdf:about="http://purl.obolibrary.org/obo/GAZ_00466217">
        <obo:IAO_0000115>A reservoir.</obo:IAO_0000115>
        <oboInOwl:hasOBONamespace>GAZ</oboInOwl:hasOBONamespace>
        <oboInOwl:id>GAZ:00466217</oboInOwl:id>
        <rdfs:label>Talsperre Horni Becva</rdfs:label>
    </owl:NamedIndividual>
    


    <!-- http://purl.obolibrary.org/obo/GAZ_00466250 -->

    <owl:NamedIndividual rdf:about="http://purl.obolibrary.org/obo/GAZ_00466250">
        <obo:RO_0001025 rdf:resource="http://purl.obolibrary.org/obo/GAZ_00465557"/>
        <obo:IAO_0000115>A protected area. It lies on the border between the Zlinsky kraj - Zlin Region and the Moravskoslezsky kraj - Moravian-Silesian Region.</obo:IAO_0000115>
        <oboInOwl:hasOBONamespace>GAZ</oboInOwl:hasOBONamespace>
        <oboInOwl:id>GAZ:00466250</oboInOwl:id>
        <rdfs:label>Narodni prirodni rezervace Radhost&apos;</rdfs:label>
    </owl:NamedIndividual>
    


    <!-- http://purl.obolibrary.org/obo/GAZ_00466251 -->

    <owl:NamedIndividual rdf:about="http://purl.obolibrary.org/obo/GAZ_00466251">
        <obo:RO_0001025 rdf:resource="http://purl.obolibrary.org/obo/GAZ_00465557"/>
        <obo:IAO_0000115>A protected area. It lies approximately 1 km north of the village of Pulcin on the southern edge of the Beskydy PLA and in the Zlinsky kraj.</obo:IAO_0000115>
        <oboInOwl:hasOBONamespace>GAZ</oboInOwl:hasOBONamespace>
        <oboInOwl:id>GAZ:00466251</oboInOwl:id>
        <rdfs:label>Narodni prirodni rezervace Pulcin - Hradisko</rdfs:label>
    </owl:NamedIndividual>
    


    <!-- http://purl.obolibrary.org/obo/GAZ_00466253 -->

    <owl:NamedIndividual rdf:about="http://purl.obolibrary.org/obo/GAZ_00466253">
        <obo:RO_0001025 rdf:resource="http://purl.obolibrary.org/obo/GAZ_00465557"/>
        <obo:IAO_0000115>A protected area. Includes primeval forest communities located on the southern slope of the Velka Cantoryje mountain massif in the Slezske Beskydy mountain range 2 km NE of the village of Nydek along the Czech - Polish border and in the east of the Moravskoslezsky kraj.</obo:IAO_0000115>
        <oboInOwl:hasOBONamespace>GAZ</oboInOwl:hasOBONamespace>
        <oboInOwl:id>GAZ:00466253</oboInOwl:id>
        <rdfs:label>Narodni prirodni rezervace Cantoria</rdfs:label>
    </owl:NamedIndividual>
    


    <!-- http://purl.obolibrary.org/obo/GAZ_00466254 -->

    <owl:NamedIndividual rdf:about="http://purl.obolibrary.org/obo/GAZ_00466254">
        <obo:RO_0001025 rdf:resource="http://purl.obolibrary.org/obo/GAZ_00465557"/>
        <obo:IAO_0000115>A protected area. It includes the summit areas of Mount Knehyne (1257 m) and the Certuv mlyn Massif (1206 m) which are divided by a shallow saddle.</obo:IAO_0000115>
        <oboInOwl:hasOBONamespace>GAZ</oboInOwl:hasOBONamespace>
        <oboInOwl:id>GAZ:00466254</oboInOwl:id>
        <rdfs:label>Narodni prirodni rezervace Knehyne - Certuv mlyn</rdfs:label>
    </owl:NamedIndividual>
    


    <!-- http://purl.obolibrary.org/obo/GAZ_00466255 -->

    <owl:NamedIndividual rdf:about="http://purl.obolibrary.org/obo/GAZ_00466255">
        <obo:RO_0001025 rdf:resource="http://purl.obolibrary.org/obo/GAZ_00465557"/>
        <obo:IAO_0000115>A protected area. It lies on the western slopes of the highest mountain in the Moravskoslezske Beskydy range.</obo:IAO_0000115>
        <oboInOwl:hasOBONamespace>GAZ</oboInOwl:hasOBONamespace>
        <oboInOwl:id>GAZ:00466255</oboInOwl:id>
        <rdfs:label>Narodni prirodni rezervace Mazak</rdfs:label>
    </owl:NamedIndividual>
    


    <!-- http://purl.obolibrary.org/obo/GAZ_00466256 -->

    <owl:NamedIndividual rdf:about="http://purl.obolibrary.org/obo/GAZ_00466256">
        <obo:RO_0001025 rdf:resource="http://purl.obolibrary.org/obo/GAZ_00465557"/>
        <obo:IAO_0000115>A protected area.It lies on the ridge and slopes of Mount Uplaz (949.6 m) and Mt. Velke Polany (893 m) about 1 km east of the centre of the village of Horni Lomna, in the Moravskoslezsky kraj.</obo:IAO_0000115>
        <oboInOwl:hasOBONamespace>GAZ</oboInOwl:hasOBONamespace>
        <oboInOwl:id>GAZ:00466256</oboInOwl:id>
        <rdfs:label>Narodni prirodni rezervace Mionsi</rdfs:label>
    </owl:NamedIndividual>
    


    <!-- http://purl.obolibrary.org/obo/GAZ_00466257 -->

    <owl:NamedIndividual rdf:about="http://purl.obolibrary.org/obo/GAZ_00466257">
        <obo:RO_0001025 rdf:resource="http://purl.obolibrary.org/obo/GAZ_00465557"/>
        <obo:IAO_0000115>A protected area. It lies on the northern slopes of Mount Lemesna (950 m) in the spring areas of the Hanzluvka stream in the Javorniky mountain range. The NNR lies between the municipality of Velke Karlovice and the Slovak border, on the territory of Beskydy PLA and in the Zlinsky kraj.</obo:IAO_0000115>
        <oboInOwl:hasOBONamespace>GAZ</oboInOwl:hasOBONamespace>
        <oboInOwl:id>GAZ:00466257</oboInOwl:id>
        <rdfs:label>Narodni prirodni rezervace Razula</rdfs:label>
    </owl:NamedIndividual>
    


    <!-- http://purl.obolibrary.org/obo/GAZ_00466258 -->

    <owl:NamedIndividual rdf:about="http://purl.obolibrary.org/obo/GAZ_00466258">
        <obo:RO_0001025 rdf:resource="http://purl.obolibrary.org/obo/GAZ_00465557"/>
        <obo:IAO_0000115>A protected area. It lies on the northern slopes of the border ridge of the Moravskoslezske Beskydy mountain range close to the mountain saddle called Bumbalka. This mountain pass lies on the Czech-Slovak border, within the Beskydy PLA and the Moravskoslezsky kraj .</obo:IAO_0000115>
        <oboInOwl:hasOBONamespace>GAZ</oboInOwl:hasOBONamespace>
        <oboInOwl:id>GAZ:00466258</oboInOwl:id>
        <rdfs:label>Narodni prirodni rezervace Salajka</rdfs:label>
    </owl:NamedIndividual>
    


    <!-- http://purl.obolibrary.org/obo/GAZ_00466259 -->

    <owl:NamedIndividual rdf:about="http://purl.obolibrary.org/obo/GAZ_00466259">
        <obo:RO_0001025 rdf:resource="http://purl.obolibrary.org/obo/GAZ_00465557"/>
        <obo:IAO_0000115>A protected area. It lies in the Podbeskydska pahorkatina Hilly Land, between the municipalities of Raskovice and Nosovice in the Moravskoslezsky kraj.</obo:IAO_0000115>
        <oboInOwl:hasOBONamespace>GAZ</oboInOwl:hasOBONamespace>
        <oboInOwl:id>GAZ:00466259</oboInOwl:id>
        <rdfs:label>Narodni prirodni pamatka Skalicka Moravka</rdfs:label>
    </owl:NamedIndividual>
    


    <!-- http://purl.obolibrary.org/obo/GAZ_00466319 -->

    <owl:NamedIndividual rdf:about="http://purl.obolibrary.org/obo/GAZ_00466319">
        <obo:RO_0001025 rdf:resource="http://purl.obolibrary.org/obo/GAZ_00179205"/>
        <obo:IAO_0000115>A protected area.</obo:IAO_0000115>
        <oboInOwl:hasOBONamespace>GAZ</oboInOwl:hasOBONamespace>
        <oboInOwl:id>GAZ:00466319</oboInOwl:id>
        <rdfs:label>Narodni prirodni rezervace Certoryje</rdfs:label>
    </owl:NamedIndividual>
    


    <!-- http://purl.obolibrary.org/obo/GAZ_00466320 -->

    <owl:NamedIndividual rdf:about="http://purl.obolibrary.org/obo/GAZ_00466320">
        <obo:RO_0001025 rdf:resource="http://purl.obolibrary.org/obo/GAZ_00179205"/>
        <obo:IAO_0000115>A protected area.</obo:IAO_0000115>
        <oboInOwl:hasOBONamespace>GAZ</oboInOwl:hasOBONamespace>
        <oboInOwl:id>GAZ:00466320</oboInOwl:id>
        <rdfs:label>Narodni prirodni rezervace Javorina</rdfs:label>
    </owl:NamedIndividual>
    


    <!-- http://purl.obolibrary.org/obo/GAZ_00466321 -->

    <owl:NamedIndividual rdf:about="http://purl.obolibrary.org/obo/GAZ_00466321">
        <obo:RO_0001025 rdf:resource="http://purl.obolibrary.org/obo/GAZ_00179205"/>
        <obo:IAO_0000115>A protected area.</obo:IAO_0000115>
        <oboInOwl:hasOBONamespace>GAZ</oboInOwl:hasOBONamespace>
        <oboInOwl:id>GAZ:00466321</oboInOwl:id>
        <rdfs:label>Narodni prirodni rezervace Jazevci</rdfs:label>
    </owl:NamedIndividual>
    


    <!-- http://purl.obolibrary.org/obo/GAZ_00466322 -->

    <owl:NamedIndividual rdf:about="http://purl.obolibrary.org/obo/GAZ_00466322">
        <obo:RO_0001025 rdf:resource="http://purl.obolibrary.org/obo/GAZ_00179205"/>
        <obo:IAO_0000115>A protected area.</obo:IAO_0000115>
        <oboInOwl:hasOBONamespace>GAZ</oboInOwl:hasOBONamespace>
        <oboInOwl:id>GAZ:00466322</oboInOwl:id>
        <rdfs:label>Narodni prirodni rezervace Porazky</rdfs:label>
    </owl:NamedIndividual>
    


    <!-- http://purl.obolibrary.org/obo/GAZ_00466323 -->

    <owl:NamedIndividual rdf:about="http://purl.obolibrary.org/obo/GAZ_00466323">
        <obo:RO_0001025 rdf:resource="http://purl.obolibrary.org/obo/GAZ_00179205"/>
        <obo:IAO_0000115>A protected area.</obo:IAO_0000115>
        <oboInOwl:hasOBONamespace>GAZ</oboInOwl:hasOBONamespace>
        <oboInOwl:id>GAZ:00466323</oboInOwl:id>
        <rdfs:label>Narodni prirodni rezervace Zahrady pod Hajem</rdfs:label>
    </owl:NamedIndividual>
    


    <!-- http://purl.obolibrary.org/obo/GAZ_00466324 -->

    <owl:NamedIndividual rdf:about="http://purl.obolibrary.org/obo/GAZ_00466324">
        <obo:RO_0001025 rdf:resource="http://purl.obolibrary.org/obo/GAZ_00179205"/>
        <obo:IAO_0000115>A protected area.</obo:IAO_0000115>
        <oboInOwl:hasOBONamespace>GAZ</oboInOwl:hasOBONamespace>
        <oboInOwl:id>GAZ:00466324</oboInOwl:id>
        <rdfs:label>Narodni prirodni pamatka Burova</rdfs:label>
    </owl:NamedIndividual>
    


    <!-- http://purl.obolibrary.org/obo/GAZ_00466325 -->

    <owl:NamedIndividual rdf:about="http://purl.obolibrary.org/obo/GAZ_00466325">
        <obo:RO_0001025 rdf:resource="http://purl.obolibrary.org/obo/GAZ_00179205"/>
        <obo:IAO_0000115>A protected area.</obo:IAO_0000115>
        <oboInOwl:hasOBONamespace>GAZ</oboInOwl:hasOBONamespace>
        <oboInOwl:id>GAZ:00466325</oboInOwl:id>
        <rdfs:label>Narodni prirodni pamatka Vate pisky</rdfs:label>
    </owl:NamedIndividual>
    


    <!-- http://purl.obolibrary.org/obo/GAZ_00466409 -->

    <owl:NamedIndividual rdf:about="http://purl.obolibrary.org/obo/GAZ_00466409">
        <obo:RO_0001025 rdf:resource="http://purl.obolibrary.org/obo/GAZ_00466014"/>
        <obo:IAO_0000115>A protected area.</obo:IAO_0000115>
        <oboInOwl:hasOBONamespace>GAZ</oboInOwl:hasOBONamespace>
        <oboInOwl:id>GAZ:00466409</oboInOwl:id>
        <rdfs:label>Narodni prirodni rezervace Cahnov - Soutok</rdfs:label>
    </owl:NamedIndividual>
    


    <!-- http://purl.obolibrary.org/obo/GAZ_00466410 -->

    <owl:NamedIndividual rdf:about="http://purl.obolibrary.org/obo/GAZ_00466410">
        <obo:RO_0001025 rdf:resource="http://purl.obolibrary.org/obo/GAZ_00466014"/>
        <obo:IAO_0000115>A protected area.</obo:IAO_0000115>
        <oboInOwl:hasOBONamespace>GAZ</oboInOwl:hasOBONamespace>
        <oboInOwl:id>GAZ:00466410</oboInOwl:id>
        <rdfs:label>Narodni prirodni rezervace Devin - Kotel - Souteska</rdfs:label>
    </owl:NamedIndividual>
    


    <!-- http://purl.obolibrary.org/obo/GAZ_00466411 -->

    <owl:NamedIndividual rdf:about="http://purl.obolibrary.org/obo/GAZ_00466411">
        <obo:RO_0001025 rdf:resource="http://purl.obolibrary.org/obo/GAZ_00466014"/>
        <obo:IAO_0000115>A protected area.</obo:IAO_0000115>
        <oboInOwl:hasOBONamespace>GAZ</oboInOwl:hasOBONamespace>
        <oboInOwl:id>GAZ:00466411</oboInOwl:id>
        <rdfs:label>Narodni prirodni rezervace Krumlovsko-rokytenske slepence</rdfs:label>
    </owl:NamedIndividual>
    


    <!-- http://purl.obolibrary.org/obo/GAZ_00466412 -->

    <owl:NamedIndividual rdf:about="http://purl.obolibrary.org/obo/GAZ_00466412">
        <obo:RO_0001025 rdf:resource="http://purl.obolibrary.org/obo/GAZ_00466014"/>
        <obo:IAO_0000115>A protected area.</obo:IAO_0000115>
        <oboInOwl:hasOBONamespace>GAZ</oboInOwl:hasOBONamespace>
        <oboInOwl:id>GAZ:00466412</oboInOwl:id>
        <rdfs:label>Narodni prirodni rezervace Krive jezero</rdfs:label>
    </owl:NamedIndividual>
    


    <!-- http://purl.obolibrary.org/obo/GAZ_00466413 -->

    <owl:NamedIndividual rdf:about="http://purl.obolibrary.org/obo/GAZ_00466413">
        <obo:RO_0001025 rdf:resource="http://purl.obolibrary.org/obo/GAZ_00466014"/>
        <obo:IAO_0000115>A protected area.</obo:IAO_0000115>
        <oboInOwl:hasOBONamespace>GAZ</oboInOwl:hasOBONamespace>
        <oboInOwl:id>GAZ:00466413</oboInOwl:id>
        <rdfs:label>Narodni prirodni rezervace Lednicke rybniky</rdfs:label>
    </owl:NamedIndividual>
    


    <!-- http://purl.obolibrary.org/obo/GAZ_00466414 -->

    <owl:NamedIndividual rdf:about="http://purl.obolibrary.org/obo/GAZ_00466414">
        <obo:RO_0001025 rdf:resource="http://purl.obolibrary.org/obo/GAZ_00466014"/>
        <obo:IAO_0000115>A protected area.</obo:IAO_0000115>
        <oboInOwl:hasOBONamespace>GAZ</oboInOwl:hasOBONamespace>
        <oboInOwl:id>GAZ:00466414</oboInOwl:id>
        <rdfs:label>Narodni prirodni rezervace Pouzdranska step - Kolby</rdfs:label>
    </owl:NamedIndividual>
    


    <!-- http://purl.obolibrary.org/obo/GAZ_00466415 -->

    <owl:NamedIndividual rdf:about="http://purl.obolibrary.org/obo/GAZ_00466415">
        <obo:RO_0001025 rdf:resource="http://purl.obolibrary.org/obo/GAZ_00466014"/>
        <obo:IAO_0000115>A protected area.</obo:IAO_0000115>
        <oboInOwl:hasOBONamespace>GAZ</oboInOwl:hasOBONamespace>
        <oboInOwl:id>GAZ:00466415</oboInOwl:id>
        <rdfs:label>Narodni prirodni rezervace Ranspurk</rdfs:label>
    </owl:NamedIndividual>
    


    <!-- http://purl.obolibrary.org/obo/GAZ_00466416 -->

    <owl:NamedIndividual rdf:about="http://purl.obolibrary.org/obo/GAZ_00466416">
        <obo:RO_0001025 rdf:resource="http://purl.obolibrary.org/obo/GAZ_00466014"/>
        <obo:IAO_0000115>A protected area.</obo:IAO_0000115>
        <oboInOwl:hasOBONamespace>GAZ</oboInOwl:hasOBONamespace>
        <oboInOwl:id>GAZ:00466416</oboInOwl:id>
        <rdfs:label>Narodni prirodni rezervace Slanisko u Nesytu</rdfs:label>
    </owl:NamedIndividual>
    


    <!-- http://purl.obolibrary.org/obo/GAZ_00466417 -->

    <owl:NamedIndividual rdf:about="http://purl.obolibrary.org/obo/GAZ_00466417">
        <obo:RO_0001025 rdf:resource="http://purl.obolibrary.org/obo/GAZ_00466014"/>
        <obo:IAO_0000115>A protected area.</obo:IAO_0000115>
        <oboInOwl:hasOBONamespace>GAZ</oboInOwl:hasOBONamespace>
        <oboInOwl:id>GAZ:00466417</oboInOwl:id>
        <rdfs:label>Narodni prirodni rezervace Tabulova, Ruzovy vrch a Kocici kamen</rdfs:label>
    </owl:NamedIndividual>
    


    <!-- http://purl.obolibrary.org/obo/GAZ_00466418 -->

    <owl:NamedIndividual rdf:about="http://purl.obolibrary.org/obo/GAZ_00466418">
        <obo:RO_0001025 rdf:resource="http://purl.obolibrary.org/obo/GAZ_00466014"/>
        <obo:IAO_0000115>A protected area.</obo:IAO_0000115>
        <oboInOwl:hasOBONamespace>GAZ</oboInOwl:hasOBONamespace>
        <oboInOwl:id>GAZ:00466418</oboInOwl:id>
        <rdfs:label>Narodni prirodni rezervace Vetrniky</rdfs:label>
    </owl:NamedIndividual>
    


    <!-- http://purl.obolibrary.org/obo/GAZ_00466419 -->

    <owl:NamedIndividual rdf:about="http://purl.obolibrary.org/obo/GAZ_00466419">
        <obo:RO_0001025 rdf:resource="http://purl.obolibrary.org/obo/GAZ_00466014"/>
        <obo:IAO_0000115>A protected area.</obo:IAO_0000115>
        <oboInOwl:hasOBONamespace>GAZ</oboInOwl:hasOBONamespace>
        <oboInOwl:id>GAZ:00466419</oboInOwl:id>
        <rdfs:label>Narodni prirodni pamatka Dunajovicke kopce</rdfs:label>
    </owl:NamedIndividual>
    


    <!-- http://purl.obolibrary.org/obo/GAZ_00466420 -->

    <owl:NamedIndividual rdf:about="http://purl.obolibrary.org/obo/GAZ_00466420">
        <obo:RO_0001025 rdf:resource="http://purl.obolibrary.org/obo/GAZ_00466014"/>
        <obo:IAO_0000115>A protected area.</obo:IAO_0000115>
        <oboInOwl:hasOBONamespace>GAZ</oboInOwl:hasOBONamespace>
        <oboInOwl:id>GAZ:00466420</oboInOwl:id>
        <rdfs:label>Narodni prirodni pamatka Malhotky</rdfs:label>
    </owl:NamedIndividual>
    


    <!-- http://purl.obolibrary.org/obo/GAZ_00466421 -->

    <owl:NamedIndividual rdf:about="http://purl.obolibrary.org/obo/GAZ_00466421">
        <obo:RO_0001025 rdf:resource="http://purl.obolibrary.org/obo/GAZ_00466014"/>
        <obo:IAO_0000115>A protected area.</obo:IAO_0000115>
        <oboInOwl:hasOBONamespace>GAZ</oboInOwl:hasOBONamespace>
        <oboInOwl:id>GAZ:00466421</oboInOwl:id>
        <rdfs:label>Narodni prirodni pamatka Miroslavske kopce</rdfs:label>
    </owl:NamedIndividual>
    


    <!-- http://purl.obolibrary.org/obo/GAZ_00466422 -->

    <owl:NamedIndividual rdf:about="http://purl.obolibrary.org/obo/GAZ_00466422">
        <obo:RO_0001025 rdf:resource="http://purl.obolibrary.org/obo/GAZ_00466014"/>
        <obo:IAO_0000115>A protected area.</obo:IAO_0000115>
        <oboInOwl:hasOBONamespace>GAZ</oboInOwl:hasOBONamespace>
        <oboInOwl:id>GAZ:00466422</oboInOwl:id>
        <rdfs:label>Narodni prirodni pamatka Na Adamcich</rdfs:label>
    </owl:NamedIndividual>
    


    <!-- http://purl.obolibrary.org/obo/GAZ_00466423 -->

    <owl:NamedIndividual rdf:about="http://purl.obolibrary.org/obo/GAZ_00466423">
        <obo:RO_0001025 rdf:resource="http://purl.obolibrary.org/obo/GAZ_00466014"/>
        <obo:IAO_0000115>A protected area.</obo:IAO_0000115>
        <oboInOwl:hasOBONamespace>GAZ</oboInOwl:hasOBONamespace>
        <oboInOwl:id>GAZ:00466423</oboInOwl:id>
        <rdfs:label>Narodni prirodni pamatka Pastvisko u Lednice</rdfs:label>
    </owl:NamedIndividual>
    


    <!-- http://purl.obolibrary.org/obo/GAZ_00466424 -->

    <owl:NamedIndividual rdf:about="http://purl.obolibrary.org/obo/GAZ_00466424">
        <obo:RO_0001025 rdf:resource="http://purl.obolibrary.org/obo/GAZ_00466014"/>
        <obo:IAO_0000115>A protected area.</obo:IAO_0000115>
        <oboInOwl:hasOBONamespace>GAZ</oboInOwl:hasOBONamespace>
        <oboInOwl:id>GAZ:00466424</oboInOwl:id>
        <rdfs:label>Narodni prirodni pamatka Rendezvous</rdfs:label>
    </owl:NamedIndividual>
    


    <!-- http://purl.obolibrary.org/obo/GAZ_00466425 -->

    <owl:NamedIndividual rdf:about="http://purl.obolibrary.org/obo/GAZ_00466425">
        <obo:RO_0001025 rdf:resource="http://purl.obolibrary.org/obo/GAZ_00466014"/>
        <obo:IAO_0000115>A protected area.</obo:IAO_0000115>
        <oboInOwl:hasOBONamespace>GAZ</oboInOwl:hasOBONamespace>
        <oboInOwl:id>GAZ:00466425</oboInOwl:id>
        <rdfs:label>Narodni prirodni pamatka Kalendar veku</rdfs:label>
    </owl:NamedIndividual>
    


    <!-- http://purl.obolibrary.org/obo/GAZ_00466426 -->

    <owl:NamedIndividual rdf:about="http://purl.obolibrary.org/obo/GAZ_00466426">
        <obo:RO_0001025 rdf:resource="http://purl.obolibrary.org/obo/GAZ_00466413"/>
        <obo:IAO_0000115>A lake; a fishpond.</obo:IAO_0000115>
        <oboInOwl:hasOBONamespace>GAZ</oboInOwl:hasOBONamespace>
        <oboInOwl:id>GAZ:00466426</oboInOwl:id>
        <rdfs:label>Nesyt rybnik</rdfs:label>
    </owl:NamedIndividual>
    


    <!-- http://purl.obolibrary.org/obo/GAZ_00466427 -->

    <owl:NamedIndividual rdf:about="http://purl.obolibrary.org/obo/GAZ_00466427">
        <obo:RO_0001025 rdf:resource="http://purl.obolibrary.org/obo/GAZ_00466413"/>
        <obo:IAO_0000115>A lake; a fishpond.</obo:IAO_0000115>
        <oboInOwl:hasOBONamespace>GAZ</oboInOwl:hasOBONamespace>
        <oboInOwl:id>GAZ:00466427</oboInOwl:id>
        <rdfs:label>Hlohovecky rybnik</rdfs:label>
    </owl:NamedIndividual>
    


    <!-- http://purl.obolibrary.org/obo/GAZ_00466428 -->

    <owl:NamedIndividual rdf:about="http://purl.obolibrary.org/obo/GAZ_00466428">
        <obo:RO_0001025 rdf:resource="http://purl.obolibrary.org/obo/GAZ_00466413"/>
        <obo:IAO_0000115>A lake; a fishpond.</obo:IAO_0000115>
        <oboInOwl:hasOBONamespace>GAZ</oboInOwl:hasOBONamespace>
        <oboInOwl:id>GAZ:00466428</oboInOwl:id>
        <rdfs:label>Prostredni rybnik</rdfs:label>
    </owl:NamedIndividual>
    


    <!-- http://purl.obolibrary.org/obo/GAZ_00466429 -->

    <owl:NamedIndividual rdf:about="http://purl.obolibrary.org/obo/GAZ_00466429">
        <obo:RO_0001025 rdf:resource="http://purl.obolibrary.org/obo/GAZ_00466413"/>
        <obo:IAO_0000115>A lake; a fishpond.</obo:IAO_0000115>
        <oboInOwl:hasOBONamespace>GAZ</oboInOwl:hasOBONamespace>
        <oboInOwl:id>GAZ:00466429</oboInOwl:id>
        <rdfs:label>Mlynsky rybnik</rdfs:label>
    </owl:NamedIndividual>
    


    <!-- http://purl.obolibrary.org/obo/GAZ_00466430 -->

    <owl:NamedIndividual rdf:about="http://purl.obolibrary.org/obo/GAZ_00466430">
        <obo:RO_0001025 rdf:resource="http://purl.obolibrary.org/obo/GAZ_00466413"/>
        <obo:IAO_0000115>A lake; a fishpond.</obo:IAO_0000115>
        <oboInOwl:hasOBONamespace>GAZ</oboInOwl:hasOBONamespace>
        <oboInOwl:id>GAZ:00466430</oboInOwl:id>
        <rdfs:label>Zamecky rybnik</rdfs:label>
    </owl:NamedIndividual>
    


    <!-- http://purl.obolibrary.org/obo/GAZ_00466431 -->

    <owl:NamedIndividual rdf:about="http://purl.obolibrary.org/obo/GAZ_00466431">
        <obo:RO_0001025 rdf:resource="http://purl.obolibrary.org/obo/GAZ_00466412"/>
        <obo:IAO_0000115>A lake.</obo:IAO_0000115>
        <oboInOwl:hasOBONamespace>GAZ</oboInOwl:hasOBONamespace>
        <oboInOwl:id>GAZ:00466431</oboInOwl:id>
        <rdfs:label>Krive jezero</rdfs:label>
    </owl:NamedIndividual>
    


    <!-- http://purl.obolibrary.org/obo/GAZ_00466465 -->

    <owl:NamedIndividual rdf:about="http://purl.obolibrary.org/obo/GAZ_00466465">
        <obo:RO_0001025 rdf:resource="http://purl.obolibrary.org/obo/GAZ_00465556"/>
        <obo:IAO_0000115>A protected area.</obo:IAO_0000115>
        <oboInOwl:hasOBONamespace>GAZ</oboInOwl:hasOBONamespace>
        <oboInOwl:id>GAZ:00466465</oboInOwl:id>
        <rdfs:label>Narodni prirodni rezervace Hurka u Hranic</rdfs:label>
    </owl:NamedIndividual>
    


    <!-- http://purl.obolibrary.org/obo/GAZ_00466466 -->

    <owl:NamedIndividual rdf:about="http://purl.obolibrary.org/obo/GAZ_00466466">
        <obo:RO_0001025 rdf:resource="http://purl.obolibrary.org/obo/GAZ_00465556"/>
        <obo:IAO_0000115>A protected area.</obo:IAO_0000115>
        <oboInOwl:hasOBONamespace>GAZ</oboInOwl:hasOBONamespace>
        <oboInOwl:id>GAZ:00466466</oboInOwl:id>
        <rdfs:label>Narodni prirodni rezervace Kaluza</rdfs:label>
    </owl:NamedIndividual>
    


    <!-- http://purl.obolibrary.org/obo/GAZ_00466467 -->

    <owl:NamedIndividual rdf:about="http://purl.obolibrary.org/obo/GAZ_00466467">
        <obo:RO_0001025 rdf:resource="http://purl.obolibrary.org/obo/GAZ_00465556"/>
        <obo:IAO_0000115>A protected area.</obo:IAO_0000115>
        <oboInOwl:hasOBONamespace>GAZ</oboInOwl:hasOBONamespace>
        <oboInOwl:id>GAZ:00466467</oboInOwl:id>
        <rdfs:label>Narodni prirodni rezervace Polanska niva</rdfs:label>
    </owl:NamedIndividual>
    


    <!-- http://purl.obolibrary.org/obo/GAZ_00466468 -->

    <owl:NamedIndividual rdf:about="http://purl.obolibrary.org/obo/GAZ_00466468">
        <obo:RO_0001025 rdf:resource="http://purl.obolibrary.org/obo/GAZ_00465556"/>
        <obo:IAO_0000115>A protected area.</obo:IAO_0000115>
        <oboInOwl:hasOBONamespace>GAZ</oboInOwl:hasOBONamespace>
        <oboInOwl:id>GAZ:00466468</oboInOwl:id>
        <rdfs:label>Narodni prirodni pamatka Landek</rdfs:label>
    </owl:NamedIndividual>
    


    <!-- http://purl.obolibrary.org/obo/GAZ_00466469 -->

    <owl:NamedIndividual rdf:about="http://purl.obolibrary.org/obo/GAZ_00466469">
        <obo:RO_0001025 rdf:resource="http://purl.obolibrary.org/obo/GAZ_00465556"/>
        <obo:IAO_0000115>A protected area.</obo:IAO_0000115>
        <oboInOwl:hasOBONamespace>GAZ</oboInOwl:hasOBONamespace>
        <oboInOwl:id>GAZ:00466469</oboInOwl:id>
        <rdfs:label>Narodni prirodni pamatka Odkryv v Kravarich</rdfs:label>
    </owl:NamedIndividual>
    


    <!-- http://purl.obolibrary.org/obo/GAZ_00466470 -->

    <owl:NamedIndividual rdf:about="http://purl.obolibrary.org/obo/GAZ_00466470">
        <obo:RO_0001025 rdf:resource="http://purl.obolibrary.org/obo/GAZ_00465556"/>
        <obo:IAO_0000115>A protected area.</obo:IAO_0000115>
        <oboInOwl:hasOBONamespace>GAZ</oboInOwl:hasOBONamespace>
        <oboInOwl:id>GAZ:00466470</oboInOwl:id>
        <rdfs:label>Narodni prirodni pamatka Sipka</rdfs:label>
    </owl:NamedIndividual>
    


    <!-- http://purl.obolibrary.org/obo/GAZ_00466471 -->

    <owl:NamedIndividual rdf:about="http://purl.obolibrary.org/obo/GAZ_00466471">
        <obo:RO_0001025 rdf:resource="http://purl.obolibrary.org/obo/GAZ_00465556"/>
        <obo:IAO_0000115>A protected area.</obo:IAO_0000115>
        <oboInOwl:hasOBONamespace>GAZ</oboInOwl:hasOBONamespace>
        <oboInOwl:id>GAZ:00466471</oboInOwl:id>
        <rdfs:label>Narodni prirodni pamatka Zbrasovske aragonitove jeskyne</rdfs:label>
    </owl:NamedIndividual>
    


    <!-- http://purl.obolibrary.org/obo/GAZ_00466472 -->

    <owl:NamedIndividual rdf:about="http://purl.obolibrary.org/obo/GAZ_00466472">
        <obo:RO_0001025 rdf:resource="http://purl.obolibrary.org/obo/GAZ_00466471"/>
        <obo:IAO_0000115>An aragonite cave system.</obo:IAO_0000115>
        <oboInOwl:hasOBONamespace>GAZ</oboInOwl:hasOBONamespace>
        <oboInOwl:id>GAZ:00466472</oboInOwl:id>
        <rdfs:label>Zbrasovske aragonitove jeskyne</rdfs:label>
    </owl:NamedIndividual>
    


    <!-- http://purl.obolibrary.org/obo/GAZ_00466556 -->

    <owl:NamedIndividual rdf:about="http://purl.obolibrary.org/obo/GAZ_00466556">
        <obo:IAO_0000115>A reservoit.</obo:IAO_0000115>
        <oboInOwl:hasOBONamespace>GAZ</oboInOwl:hasOBONamespace>
        <oboInOwl:id>GAZ:00466556</oboInOwl:id>
        <rdfs:label>Vodni nadrz Zermanice</rdfs:label>
    </owl:NamedIndividual>
    


    <!-- http://purl.obolibrary.org/obo/GAZ_00466626 -->

    <owl:NamedIndividual rdf:about="http://purl.obolibrary.org/obo/GAZ_00466626">
        <obo:RO_0001025 rdf:resource="http://purl.obolibrary.org/obo/GAZ_00465557"/>
        <obo:IAO_0000115>A protected area.</obo:IAO_0000115>
        <oboInOwl:hasOBONamespace>GAZ</oboInOwl:hasOBONamespace>
        <oboInOwl:id>GAZ:00466626</oboInOwl:id>
        <rdfs:label>Prirodni rezervace Bucaci potok</rdfs:label>
    </owl:NamedIndividual>
    


    <!-- http://purl.obolibrary.org/obo/GAZ_00466627 -->

    <owl:NamedIndividual rdf:about="http://purl.obolibrary.org/obo/GAZ_00466627">
        <obo:RO_0001025 rdf:resource="http://purl.obolibrary.org/obo/GAZ_00465557"/>
        <obo:IAO_0000115>A protected area.</obo:IAO_0000115>
        <oboInOwl:hasOBONamespace>GAZ</oboInOwl:hasOBONamespace>
        <oboInOwl:id>GAZ:00466627</oboInOwl:id>
        <rdfs:label>Prirodni rezervace Cernavina</rdfs:label>
    </owl:NamedIndividual>
    


    <!-- http://purl.obolibrary.org/obo/GAZ_00466628 -->

    <owl:NamedIndividual rdf:about="http://purl.obolibrary.org/obo/GAZ_00466628">
        <obo:RO_0001025 rdf:resource="http://purl.obolibrary.org/obo/GAZ_00465557"/>
        <obo:IAO_0000115>A protected area.</obo:IAO_0000115>
        <oboInOwl:hasOBONamespace>GAZ</oboInOwl:hasOBONamespace>
        <oboInOwl:id>GAZ:00466628</oboInOwl:id>
        <rdfs:label>Prirodni rezervace Draplavy</rdfs:label>
    </owl:NamedIndividual>
    


    <!-- http://purl.obolibrary.org/obo/GAZ_00466629 -->

    <owl:NamedIndividual rdf:about="http://purl.obolibrary.org/obo/GAZ_00466629">
        <obo:RO_0001025 rdf:resource="http://purl.obolibrary.org/obo/GAZ_00465557"/>
        <obo:IAO_0000115>A protected area.</obo:IAO_0000115>
        <oboInOwl:hasOBONamespace>GAZ</oboInOwl:hasOBONamespace>
        <oboInOwl:id>GAZ:00466629</oboInOwl:id>
        <rdfs:label>Prirodni rezervace Galovske luky</rdfs:label>
    </owl:NamedIndividual>
    


    <!-- http://purl.obolibrary.org/obo/GAZ_00466630 -->

    <owl:NamedIndividual rdf:about="http://purl.obolibrary.org/obo/GAZ_00466630">
        <obo:RO_0001025 rdf:resource="http://purl.obolibrary.org/obo/GAZ_00465557"/>
        <obo:IAO_0000115>A protected area.</obo:IAO_0000115>
        <oboInOwl:hasOBONamespace>GAZ</oboInOwl:hasOBONamespace>
        <oboInOwl:id>GAZ:00466630</oboInOwl:id>
        <rdfs:label>Prirodni rezervace Hustyn</rdfs:label>
    </owl:NamedIndividual>
    


    <!-- http://purl.obolibrary.org/obo/GAZ_00466631 -->

    <owl:NamedIndividual rdf:about="http://purl.obolibrary.org/obo/GAZ_00466631">
        <obo:RO_0001025 rdf:resource="http://purl.obolibrary.org/obo/GAZ_00465557"/>
        <obo:IAO_0000115>A protected area.</obo:IAO_0000115>
        <oboInOwl:hasOBONamespace>GAZ</oboInOwl:hasOBONamespace>
        <oboInOwl:id>GAZ:00466631</oboInOwl:id>
        <rdfs:label>Prirodni rezervace Kliny</rdfs:label>
    </owl:NamedIndividual>
    


    <!-- http://purl.obolibrary.org/obo/GAZ_00466632 -->

    <owl:NamedIndividual rdf:about="http://purl.obolibrary.org/obo/GAZ_00466632">
        <obo:RO_0001025 rdf:resource="http://purl.obolibrary.org/obo/GAZ_00465557"/>
        <obo:IAO_0000115>A protected area.</obo:IAO_0000115>
        <oboInOwl:hasOBONamespace>GAZ</oboInOwl:hasOBONamespace>
        <oboInOwl:id>GAZ:00466632</oboInOwl:id>
        <rdfs:label>Prirodni rezervace Kutany</rdfs:label>
    </owl:NamedIndividual>
    


    <!-- http://purl.obolibrary.org/obo/GAZ_00466633 -->

    <owl:NamedIndividual rdf:about="http://purl.obolibrary.org/obo/GAZ_00466633">
        <obo:RO_0001025 rdf:resource="http://purl.obolibrary.org/obo/GAZ_00465557"/>
        <obo:IAO_0000115>A protected area.</obo:IAO_0000115>
        <oboInOwl:hasOBONamespace>GAZ</oboInOwl:hasOBONamespace>
        <oboInOwl:id>GAZ:00466633</oboInOwl:id>
        <rdfs:label>Prirodni rezervace Malenovicky kotel</rdfs:label>
    </owl:NamedIndividual>
    


    <!-- http://purl.obolibrary.org/obo/GAZ_00466634 -->

    <owl:NamedIndividual rdf:about="http://purl.obolibrary.org/obo/GAZ_00466634">
        <obo:RO_0001025 rdf:resource="http://purl.obolibrary.org/obo/GAZ_00465557"/>
        <obo:IAO_0000115>A protected area.</obo:IAO_0000115>
        <oboInOwl:hasOBONamespace>GAZ</oboInOwl:hasOBONamespace>
        <oboInOwl:id>GAZ:00466634</oboInOwl:id>
        <rdfs:label>Prirodni rezervace Maly Smrk</rdfs:label>
    </owl:NamedIndividual>
    


    <!-- http://purl.obolibrary.org/obo/GAZ_00466635 -->

    <owl:NamedIndividual rdf:about="http://purl.obolibrary.org/obo/GAZ_00466635">
        <obo:RO_0001025 rdf:resource="http://purl.obolibrary.org/obo/GAZ_00465557"/>
        <obo:IAO_0000115>A protected area.</obo:IAO_0000115>
        <oboInOwl:hasOBONamespace>GAZ</oboInOwl:hasOBONamespace>
        <oboInOwl:id>GAZ:00466635</oboInOwl:id>
        <rdfs:label>Prirodni rezervace Mazacky Grunik</rdfs:label>
    </owl:NamedIndividual>
    


    <!-- http://purl.obolibrary.org/obo/GAZ_00466636 -->

    <owl:NamedIndividual rdf:about="http://purl.obolibrary.org/obo/GAZ_00466636">
        <obo:RO_0001025 rdf:resource="http://purl.obolibrary.org/obo/GAZ_00465557"/>
        <obo:IAO_0000115>A protected area.</obo:IAO_0000115>
        <oboInOwl:hasOBONamespace>GAZ</oboInOwl:hasOBONamespace>
        <oboInOwl:id>GAZ:00466636</oboInOwl:id>
        <rdfs:label>Prirodni rezervace Norici</rdfs:label>
    </owl:NamedIndividual>
    


    <!-- http://purl.obolibrary.org/obo/GAZ_00466637 -->

    <owl:NamedIndividual rdf:about="http://purl.obolibrary.org/obo/GAZ_00466637">
        <obo:RO_0001025 rdf:resource="http://purl.obolibrary.org/obo/GAZ_00465557"/>
        <obo:IAO_0000115>A protected area.</obo:IAO_0000115>
        <oboInOwl:hasOBONamespace>GAZ</oboInOwl:hasOBONamespace>
        <oboInOwl:id>GAZ:00466637</oboInOwl:id>
        <rdfs:label>Prirodni rezervace Polednana</rdfs:label>
    </owl:NamedIndividual>
    


    <!-- http://purl.obolibrary.org/obo/GAZ_00466638 -->

    <owl:NamedIndividual rdf:about="http://purl.obolibrary.org/obo/GAZ_00466638">
        <obo:RO_0001025 rdf:resource="http://purl.obolibrary.org/obo/GAZ_00465557"/>
        <obo:IAO_0000115>A protected area.</obo:IAO_0000115>
        <oboInOwl:hasOBONamespace>GAZ</oboInOwl:hasOBONamespace>
        <oboInOwl:id>GAZ:00466638</oboInOwl:id>
        <rdfs:label>Prirodni rezervace Smrk</rdfs:label>
    </owl:NamedIndividual>
    


    <!-- http://purl.obolibrary.org/obo/GAZ_00466639 -->

    <owl:NamedIndividual rdf:about="http://purl.obolibrary.org/obo/GAZ_00466639">
        <obo:RO_0001025 rdf:resource="http://purl.obolibrary.org/obo/GAZ_00465557"/>
        <obo:IAO_0000115>A protected area.</obo:IAO_0000115>
        <oboInOwl:hasOBONamespace>GAZ</oboInOwl:hasOBONamespace>
        <oboInOwl:id>GAZ:00466639</oboInOwl:id>
        <rdfs:label>Prirodni rezervace Studencany</rdfs:label>
    </owl:NamedIndividual>
    


    <!-- http://purl.obolibrary.org/obo/GAZ_00466640 -->

    <owl:NamedIndividual rdf:about="http://purl.obolibrary.org/obo/GAZ_00466640">
        <obo:RO_0001025 rdf:resource="http://purl.obolibrary.org/obo/GAZ_00465557"/>
        <obo:IAO_0000115>A protected area.</obo:IAO_0000115>
        <oboInOwl:hasOBONamespace>GAZ</oboInOwl:hasOBONamespace>
        <oboInOwl:id>GAZ:00466640</oboInOwl:id>
        <rdfs:label>Prirodni rezervace Travny</rdfs:label>
    </owl:NamedIndividual>
    


    <!-- http://purl.obolibrary.org/obo/GAZ_00466641 -->

    <owl:NamedIndividual rdf:about="http://purl.obolibrary.org/obo/GAZ_00466641">
        <obo:RO_0001025 rdf:resource="http://purl.obolibrary.org/obo/GAZ_00465557"/>
        <obo:IAO_0000115>A protected area.</obo:IAO_0000115>
        <oboInOwl:hasOBONamespace>GAZ</oboInOwl:hasOBONamespace>
        <oboInOwl:id>GAZ:00466641</oboInOwl:id>
        <rdfs:label>Prirodni rezervace Travny potok</rdfs:label>
    </owl:NamedIndividual>
    


    <!-- http://purl.obolibrary.org/obo/GAZ_00466642 -->

    <owl:NamedIndividual rdf:about="http://purl.obolibrary.org/obo/GAZ_00466642">
        <obo:RO_0001025 rdf:resource="http://purl.obolibrary.org/obo/GAZ_00465557"/>
        <obo:IAO_0000115>A protected area.</obo:IAO_0000115>
        <oboInOwl:hasOBONamespace>GAZ</oboInOwl:hasOBONamespace>
        <oboInOwl:id>GAZ:00466642</oboInOwl:id>
        <rdfs:label>Prirodni rezervace Trojacka</rdfs:label>
    </owl:NamedIndividual>
    


    <!-- http://purl.obolibrary.org/obo/GAZ_00466643 -->

    <owl:NamedIndividual rdf:about="http://purl.obolibrary.org/obo/GAZ_00466643">
        <obo:RO_0001025 rdf:resource="http://purl.obolibrary.org/obo/GAZ_00465557"/>
        <obo:IAO_0000115>A protected area.</obo:IAO_0000115>
        <oboInOwl:hasOBONamespace>GAZ</oboInOwl:hasOBONamespace>
        <oboInOwl:id>GAZ:00466643</oboInOwl:id>
        <rdfs:label>Prirodni rezervace V Podolankach</rdfs:label>
    </owl:NamedIndividual>
    


    <!-- http://purl.obolibrary.org/obo/GAZ_00466644 -->

    <owl:NamedIndividual rdf:about="http://purl.obolibrary.org/obo/GAZ_00466644">
        <obo:RO_0001025 rdf:resource="http://purl.obolibrary.org/obo/GAZ_00465557"/>
        <obo:IAO_0000115>A protected area.</obo:IAO_0000115>
        <oboInOwl:hasOBONamespace>GAZ</oboInOwl:hasOBONamespace>
        <oboInOwl:id>GAZ:00466644</oboInOwl:id>
        <rdfs:label>Prirodni rezervace Velky Polom</rdfs:label>
    </owl:NamedIndividual>
    


    <!-- http://purl.obolibrary.org/obo/GAZ_00466645 -->

    <owl:NamedIndividual rdf:about="http://purl.obolibrary.org/obo/GAZ_00466645">
        <obo:RO_0001025 rdf:resource="http://purl.obolibrary.org/obo/GAZ_00465557"/>
        <obo:IAO_0000115>A protected area.</obo:IAO_0000115>
        <oboInOwl:hasOBONamespace>GAZ</oboInOwl:hasOBONamespace>
        <oboInOwl:id>GAZ:00466645</oboInOwl:id>
        <rdfs:label>Prirodni rezervace Zimny potok</rdfs:label>
    </owl:NamedIndividual>
    


    <!-- http://purl.obolibrary.org/obo/GAZ_00466646 -->

    <owl:NamedIndividual rdf:about="http://purl.obolibrary.org/obo/GAZ_00466646">
        <obo:RO_0001025 rdf:resource="http://purl.obolibrary.org/obo/GAZ_00465557"/>
        <obo:IAO_0000115>A protected area.</obo:IAO_0000115>
        <oboInOwl:hasOBONamespace>GAZ</oboInOwl:hasOBONamespace>
        <oboInOwl:id>GAZ:00466646</oboInOwl:id>
        <rdfs:label>Prirodni pamatka Brodska</rdfs:label>
    </owl:NamedIndividual>
    


    <!-- http://purl.obolibrary.org/obo/GAZ_00466647 -->

    <owl:NamedIndividual rdf:about="http://purl.obolibrary.org/obo/GAZ_00466647">
        <obo:RO_0001025 rdf:resource="http://purl.obolibrary.org/obo/GAZ_00465557"/>
        <obo:IAO_0000115>A protected area.</obo:IAO_0000115>
        <oboInOwl:hasOBONamespace>GAZ</oboInOwl:hasOBONamespace>
        <oboInOwl:id>GAZ:00466647</oboInOwl:id>
        <rdfs:label>Prirodni pamatka Bycinec</rdfs:label>
    </owl:NamedIndividual>
    


    <!-- http://purl.obolibrary.org/obo/GAZ_00466648 -->

    <owl:NamedIndividual rdf:about="http://purl.obolibrary.org/obo/GAZ_00466648">
        <obo:RO_0001025 rdf:resource="http://purl.obolibrary.org/obo/GAZ_00465557"/>
        <obo:IAO_0000115>A protected area.</obo:IAO_0000115>
        <oboInOwl:hasOBONamespace>GAZ</oboInOwl:hasOBONamespace>
        <oboInOwl:id>GAZ:00466648</oboInOwl:id>
        <rdfs:label>Prirodni pamatka Kladnata - Grapy</rdfs:label>
    </owl:NamedIndividual>
    


    <!-- http://purl.obolibrary.org/obo/GAZ_00466649 -->

    <owl:NamedIndividual rdf:about="http://purl.obolibrary.org/obo/GAZ_00466649">
        <obo:RO_0001025 rdf:resource="http://purl.obolibrary.org/obo/GAZ_00465557"/>
        <obo:IAO_0000115>A protected area.</obo:IAO_0000115>
        <oboInOwl:hasOBONamespace>GAZ</oboInOwl:hasOBONamespace>
        <oboInOwl:id>GAZ:00466649</oboInOwl:id>
        <rdfs:label>Prirodni pamatka Knehynska jeskyne</rdfs:label>
    </owl:NamedIndividual>
    


    <!-- http://purl.obolibrary.org/obo/GAZ_00466650 -->

    <owl:NamedIndividual rdf:about="http://purl.obolibrary.org/obo/GAZ_00466650">
        <obo:RO_0001025 rdf:resource="http://purl.obolibrary.org/obo/GAZ_00465557"/>
        <obo:IAO_0000115>A protected area.</obo:IAO_0000115>
        <oboInOwl:hasOBONamespace>GAZ</oboInOwl:hasOBONamespace>
        <oboInOwl:id>GAZ:00466650</oboInOwl:id>
        <rdfs:label>Prirodni pamatka Kudlacena</rdfs:label>
    </owl:NamedIndividual>
    


    <!-- http://purl.obolibrary.org/obo/GAZ_00466651 -->

    <owl:NamedIndividual rdf:about="http://purl.obolibrary.org/obo/GAZ_00466651">
        <obo:RO_0001025 rdf:resource="http://purl.obolibrary.org/obo/GAZ_00465557"/>
        <obo:IAO_0000115>A protected area.</obo:IAO_0000115>
        <oboInOwl:hasOBONamespace>GAZ</oboInOwl:hasOBONamespace>
        <oboInOwl:id>GAZ:00466651</oboInOwl:id>
        <rdfs:label>Prirodni pamatka Kycmol</rdfs:label>
    </owl:NamedIndividual>
    


    <!-- http://purl.obolibrary.org/obo/GAZ_00466652 -->

    <owl:NamedIndividual rdf:about="http://purl.obolibrary.org/obo/GAZ_00466652">
        <obo:RO_0001025 rdf:resource="http://purl.obolibrary.org/obo/GAZ_00465557"/>
        <obo:IAO_0000115>A protected area.</obo:IAO_0000115>
        <oboInOwl:hasOBONamespace>GAZ</oboInOwl:hasOBONamespace>
        <oboInOwl:id>GAZ:00466652</oboInOwl:id>
        <rdfs:label>Prirodni pamatka Liskova</rdfs:label>
    </owl:NamedIndividual>
    


    <!-- http://purl.obolibrary.org/obo/GAZ_00466653 -->

    <owl:NamedIndividual rdf:about="http://purl.obolibrary.org/obo/GAZ_00466653">
        <obo:RO_0001025 rdf:resource="http://purl.obolibrary.org/obo/GAZ_00465557"/>
        <obo:IAO_0000115>A protected area.</obo:IAO_0000115>
        <oboInOwl:hasOBONamespace>GAZ</oboInOwl:hasOBONamespace>
        <oboInOwl:id>GAZ:00466653</oboInOwl:id>
        <rdfs:label>Prirodni pamatka Motycanka</rdfs:label>
    </owl:NamedIndividual>
    


    <!-- http://purl.obolibrary.org/obo/GAZ_00466654 -->

    <owl:NamedIndividual rdf:about="http://purl.obolibrary.org/obo/GAZ_00466654">
        <obo:RO_0001025 rdf:resource="http://purl.obolibrary.org/obo/GAZ_00465557"/>
        <obo:IAO_0000115>A protected area.</obo:IAO_0000115>
        <oboInOwl:hasOBONamespace>GAZ</oboInOwl:hasOBONamespace>
        <oboInOwl:id>GAZ:00466654</oboInOwl:id>
        <rdfs:label>Prirodni pamatka Obidova</rdfs:label>
    </owl:NamedIndividual>
    


    <!-- http://purl.obolibrary.org/obo/GAZ_00466655 -->

    <owl:NamedIndividual rdf:about="http://purl.obolibrary.org/obo/GAZ_00466655">
        <obo:RO_0001025 rdf:resource="http://purl.obolibrary.org/obo/GAZ_00465557"/>
        <obo:IAO_0000115>A protected area.</obo:IAO_0000115>
        <oboInOwl:hasOBONamespace>GAZ</oboInOwl:hasOBONamespace>
        <oboInOwl:id>GAZ:00466655</oboInOwl:id>
        <rdfs:label>Prirodni pamatka Ondrasovy diry</rdfs:label>
    </owl:NamedIndividual>
    


    <!-- http://purl.obolibrary.org/obo/GAZ_00466656 -->

    <owl:NamedIndividual rdf:about="http://purl.obolibrary.org/obo/GAZ_00466656">
        <obo:RO_0001025 rdf:resource="http://purl.obolibrary.org/obo/GAZ_00465557"/>
        <obo:IAO_0000115>A protected area.</obo:IAO_0000115>
        <oboInOwl:hasOBONamespace>GAZ</oboInOwl:hasOBONamespace>
        <oboInOwl:id>GAZ:00466656</oboInOwl:id>
        <rdfs:label>Prirodni pamatka Pod Juraskou</rdfs:label>
    </owl:NamedIndividual>
    


    <!-- http://purl.obolibrary.org/obo/GAZ_00466657 -->

    <owl:NamedIndividual rdf:about="http://purl.obolibrary.org/obo/GAZ_00466657">
        <obo:RO_0001025 rdf:resource="http://purl.obolibrary.org/obo/GAZ_00465557"/>
        <obo:IAO_0000115>A protected area.</obo:IAO_0000115>
        <oboInOwl:hasOBONamespace>GAZ</oboInOwl:hasOBONamespace>
        <oboInOwl:id>GAZ:00466657</oboInOwl:id>
        <rdfs:label>Prirodni pamatka Pod Luksincem</rdfs:label>
    </owl:NamedIndividual>
    


    <!-- http://purl.obolibrary.org/obo/GAZ_00466658 -->

    <owl:NamedIndividual rdf:about="http://purl.obolibrary.org/obo/GAZ_00466658">
        <obo:RO_0001025 rdf:resource="http://purl.obolibrary.org/obo/GAZ_00465557"/>
        <obo:IAO_0000115>A protected area.</obo:IAO_0000115>
        <oboInOwl:hasOBONamespace>GAZ</oboInOwl:hasOBONamespace>
        <oboInOwl:id>GAZ:00466658</oboInOwl:id>
        <rdfs:label>Prirodni pamatka Podgrun</rdfs:label>
    </owl:NamedIndividual>
    


    <!-- http://purl.obolibrary.org/obo/GAZ_00466659 -->

    <owl:NamedIndividual rdf:about="http://purl.obolibrary.org/obo/GAZ_00466659">
        <obo:RO_0001025 rdf:resource="http://purl.obolibrary.org/obo/GAZ_00465557"/>
        <obo:IAO_0000115>A protected area.</obo:IAO_0000115>
        <oboInOwl:hasOBONamespace>GAZ</oboInOwl:hasOBONamespace>
        <oboInOwl:id>GAZ:00466659</oboInOwl:id>
        <rdfs:label>Prirodni pamatka Poskla</rdfs:label>
    </owl:NamedIndividual>
    


    <!-- http://purl.obolibrary.org/obo/GAZ_00466660 -->

    <owl:NamedIndividual rdf:about="http://purl.obolibrary.org/obo/GAZ_00466660">
        <obo:RO_0001025 rdf:resource="http://purl.obolibrary.org/obo/GAZ_00465557"/>
        <obo:IAO_0000115>A protected area.</obo:IAO_0000115>
        <oboInOwl:hasOBONamespace>GAZ</oboInOwl:hasOBONamespace>
        <oboInOwl:id>GAZ:00466660</oboInOwl:id>
        <rdfs:label>Prirodni pamatka Rakosina Stritez</rdfs:label>
    </owl:NamedIndividual>
    


    <!-- http://purl.obolibrary.org/obo/GAZ_00466661 -->

    <owl:NamedIndividual rdf:about="http://purl.obolibrary.org/obo/GAZ_00466661">
        <obo:RO_0001025 rdf:resource="http://purl.obolibrary.org/obo/GAZ_00465557"/>
        <obo:IAO_0000115>A protected area.</obo:IAO_0000115>
        <oboInOwl:hasOBONamespace>GAZ</oboInOwl:hasOBONamespace>
        <oboInOwl:id>GAZ:00466661</oboInOwl:id>
        <rdfs:label>Prirodni pamatka Skali</rdfs:label>
    </owl:NamedIndividual>
    


    <!-- http://purl.obolibrary.org/obo/GAZ_00466662 -->

    <owl:NamedIndividual rdf:about="http://purl.obolibrary.org/obo/GAZ_00466662">
        <obo:RO_0001025 rdf:resource="http://purl.obolibrary.org/obo/GAZ_00465557"/>
        <obo:IAO_0000115>A protected area.</obo:IAO_0000115>
        <oboInOwl:hasOBONamespace>GAZ</oboInOwl:hasOBONamespace>
        <oboInOwl:id>GAZ:00466662</oboInOwl:id>
        <rdfs:label>Prirodni pamatka Smradlava</rdfs:label>
    </owl:NamedIndividual>
    


    <!-- http://purl.obolibrary.org/obo/GAZ_00466663 -->

    <owl:NamedIndividual rdf:about="http://purl.obolibrary.org/obo/GAZ_00466663">
        <obo:RO_0001025 rdf:resource="http://purl.obolibrary.org/obo/GAZ_00465557"/>
        <obo:IAO_0000115>A protected area.</obo:IAO_0000115>
        <oboInOwl:hasOBONamespace>GAZ</oboInOwl:hasOBONamespace>
        <oboInOwl:id>GAZ:00466663</oboInOwl:id>
        <rdfs:label>Prirodni pamatka Stribrnik</rdfs:label>
    </owl:NamedIndividual>
    


    <!-- http://purl.obolibrary.org/obo/GAZ_00466664 -->

    <owl:NamedIndividual rdf:about="http://purl.obolibrary.org/obo/GAZ_00466664">
        <obo:RO_0001025 rdf:resource="http://purl.obolibrary.org/obo/GAZ_00465557"/>
        <obo:IAO_0000115>A protected area.</obo:IAO_0000115>
        <oboInOwl:hasOBONamespace>GAZ</oboInOwl:hasOBONamespace>
        <oboInOwl:id>GAZ:00466664</oboInOwl:id>
        <rdfs:label>Prirodni pamatka Uherska</rdfs:label>
    </owl:NamedIndividual>
    


    <!-- http://purl.obolibrary.org/obo/GAZ_00466665 -->

    <owl:NamedIndividual rdf:about="http://purl.obolibrary.org/obo/GAZ_00466665">
        <obo:RO_0001025 rdf:resource="http://purl.obolibrary.org/obo/GAZ_00465557"/>
        <obo:IAO_0000115>A protected area.</obo:IAO_0000115>
        <oboInOwl:hasOBONamespace>GAZ</oboInOwl:hasOBONamespace>
        <oboInOwl:id>GAZ:00466665</oboInOwl:id>
        <rdfs:label>Prirodni pamatka Vachalka</rdfs:label>
    </owl:NamedIndividual>
    


    <!-- http://purl.obolibrary.org/obo/GAZ_00466666 -->

    <owl:NamedIndividual rdf:about="http://purl.obolibrary.org/obo/GAZ_00466666">
        <obo:RO_0001025 rdf:resource="http://purl.obolibrary.org/obo/GAZ_00465557"/>
        <obo:IAO_0000115>A protected area.</obo:IAO_0000115>
        <oboInOwl:hasOBONamespace>GAZ</oboInOwl:hasOBONamespace>
        <oboInOwl:id>GAZ:00466666</oboInOwl:id>
        <rdfs:label>Prirodni pamatka Velky kamen</rdfs:label>
    </owl:NamedIndividual>
    


    <!-- http://purl.obolibrary.org/obo/GAZ_00466667 -->

    <owl:NamedIndividual rdf:about="http://purl.obolibrary.org/obo/GAZ_00466667">
        <obo:RO_0001025 rdf:resource="http://purl.obolibrary.org/obo/GAZ_00465557"/>
        <obo:IAO_0000115>A protected area.</obo:IAO_0000115>
        <oboInOwl:hasOBONamespace>GAZ</oboInOwl:hasOBONamespace>
        <oboInOwl:id>GAZ:00466667</oboInOwl:id>
        <rdfs:label>Prirodni pamatka Vodopady Satiny</rdfs:label>
    </owl:NamedIndividual>
    


    <!-- http://purl.obolibrary.org/obo/GAZ_00466668 -->

    <owl:NamedIndividual rdf:about="http://purl.obolibrary.org/obo/GAZ_00466668">
        <obo:RO_0001025 rdf:resource="http://purl.obolibrary.org/obo/GAZ_00465557"/>
        <obo:IAO_0000115>A protected area.</obo:IAO_0000115>
        <oboInOwl:hasOBONamespace>GAZ</oboInOwl:hasOBONamespace>
        <oboInOwl:id>GAZ:00466668</oboInOwl:id>
        <rdfs:label>Prirodni pamatka Zubri</rdfs:label>
    </owl:NamedIndividual>
    


    <!-- http://purl.obolibrary.org/obo/GAZ_00466711 -->

    <owl:NamedIndividual rdf:about="http://purl.obolibrary.org/obo/GAZ_00466711">
        <obo:RO_0001025 rdf:resource="http://purl.obolibrary.org/obo/GAZ_00466014"/>
        <obo:IAO_0000115>A cave system.</obo:IAO_0000115>
        <oboInOwl:hasOBONamespace>GAZ</oboInOwl:hasOBONamespace>
        <oboInOwl:id>GAZ:00466711</oboInOwl:id>
        <rdfs:label>Jeskyne Na Turoldu</rdfs:label>
    </owl:NamedIndividual>
    


    <!-- http://purl.obolibrary.org/obo/GAZ_00466712 -->

    <owl:NamedIndividual rdf:about="http://purl.obolibrary.org/obo/GAZ_00466712">
        <obo:RO_0001025 rdf:resource="http://purl.obolibrary.org/obo/GAZ_00466711"/>
        <obo:IAO_0000115>A cave.</obo:IAO_0000115>
        <oboInOwl:hasOBONamespace>GAZ</oboInOwl:hasOBONamespace>
        <oboInOwl:id>GAZ:00466712</oboInOwl:id>
        <rdfs:label>Lisci dira</rdfs:label>
    </owl:NamedIndividual>
    


    <!-- http://purl.obolibrary.org/obo/GAZ_00466763 -->

    <owl:NamedIndividual rdf:about="http://purl.obolibrary.org/obo/GAZ_00466763">
        <obo:RO_0001025 rdf:resource="http://purl.obolibrary.org/obo/GAZ_00466655"/>
        <obo:IAO_0000115>A cave system.</obo:IAO_0000115>
        <oboInOwl:hasOBONamespace>GAZ</oboInOwl:hasOBONamespace>
        <oboInOwl:id>GAZ:00466763</oboInOwl:id>
        <rdfs:label>Ondrasovy diry</rdfs:label>
    </owl:NamedIndividual>
    


    <!-- http://purl.obolibrary.org/obo/GAZ_00466852 -->

    <owl:NamedIndividual rdf:about="http://purl.obolibrary.org/obo/GAZ_00466852">
        <obo:IAO_0000115>A karst lake.</obo:IAO_0000115>
        <oboInOwl:hasOBONamespace>GAZ</oboInOwl:hasOBONamespace>
        <oboInOwl:id>GAZ:00466852</oboInOwl:id>
        <rdfs:label>Dolni macosske jezirko</rdfs:label>
    </owl:NamedIndividual>
    


    <!-- http://purl.obolibrary.org/obo/GAZ_00466886 -->

    <owl:NamedIndividual rdf:about="http://purl.obolibrary.org/obo/GAZ_00466886">
        <obo:RO_0001025 rdf:resource="http://purl.obolibrary.org/obo/GAZ_00148563"/>
        <obo:IAO_0000115>A river.</obo:IAO_0000115>
        <oboInOwl:hasOBONamespace>GAZ</oboInOwl:hasOBONamespace>
        <oboInOwl:id>GAZ:00466886</oboInOwl:id>
        <rdfs:label>Prunerovsky potok</rdfs:label>
    </owl:NamedIndividual>
    


    <!-- http://purl.obolibrary.org/obo/GAZ_00466890 -->

    <owl:NamedIndividual rdf:about="http://purl.obolibrary.org/obo/GAZ_00466890">
        <obo:IAO_0000115>A river.</obo:IAO_0000115>
        <oboInOwl:hasOBONamespace>GAZ</oboInOwl:hasOBONamespace>
        <oboInOwl:id>GAZ:00466890</oboInOwl:id>
        <rdfs:label>Schwarzwasser</rdfs:label>
    </owl:NamedIndividual>
    


    <!-- http://purl.obolibrary.org/obo/GAZ_00467178 -->

    <owl:NamedIndividual rdf:about="http://purl.obolibrary.org/obo/GAZ_00467178">
        <obo:IAO_0000115>A reservoir.</obo:IAO_0000115>
        <oboInOwl:hasOBONamespace>GAZ</oboInOwl:hasOBONamespace>
        <oboInOwl:id>GAZ:00467178</oboInOwl:id>
        <rdfs:label>Vodna nadrz v Brne</rdfs:label>
    </owl:NamedIndividual>
    


    <!-- http://purl.obolibrary.org/obo/GAZ_00467179 -->

    <owl:NamedIndividual rdf:about="http://purl.obolibrary.org/obo/GAZ_00467179">
        <obo:IAO_0000115>A resrervoir.</obo:IAO_0000115>
        <oboInOwl:hasOBONamespace>GAZ</oboInOwl:hasOBONamespace>
        <oboInOwl:id>GAZ:00467179</oboInOwl:id>
        <rdfs:label>Vodni nadrz Letovice</rdfs:label>
    </owl:NamedIndividual>
    


    <!-- http://purl.obolibrary.org/obo/GAZ_00467180 -->

    <owl:NamedIndividual rdf:about="http://purl.obolibrary.org/obo/GAZ_00467180">
        <obo:IAO_0000115>A reservoir.</obo:IAO_0000115>
        <oboInOwl:hasOBONamespace>GAZ</oboInOwl:hasOBONamespace>
        <oboInOwl:id>GAZ:00467180</oboInOwl:id>
        <rdfs:label>Vodni nadrz Opatovice</rdfs:label>
    </owl:NamedIndividual>
    


    <!-- http://purl.obolibrary.org/obo/GAZ_00467181 -->

    <owl:NamedIndividual rdf:about="http://purl.obolibrary.org/obo/GAZ_00467181">
        <obo:IAO_0000115>A reservoir.</obo:IAO_0000115>
        <oboInOwl:hasOBONamespace>GAZ</oboInOwl:hasOBONamespace>
        <oboInOwl:id>GAZ:00467181</oboInOwl:id>
        <rdfs:label>Vodni nadrz Boskovice</rdfs:label>
    </owl:NamedIndividual>
    


    <!-- http://purl.obolibrary.org/obo/GAZ_00467182 -->

    <owl:NamedIndividual rdf:about="http://purl.obolibrary.org/obo/GAZ_00467182">
        <obo:IAO_0000115>A reservoir.</obo:IAO_0000115>
        <oboInOwl:hasOBONamespace>GAZ</oboInOwl:hasOBONamespace>
        <oboInOwl:id>GAZ:00467182</oboInOwl:id>
        <rdfs:label>Vodni nadrz Vranov</rdfs:label>
    </owl:NamedIndividual>
    


    <!-- http://purl.obolibrary.org/obo/GAZ_00467183 -->

    <owl:NamedIndividual rdf:about="http://purl.obolibrary.org/obo/GAZ_00467183">
        <oboInOwl:hasOBONamespace>GAZ</oboInOwl:hasOBONamespace>
        <oboInOwl:id>GAZ:00467183</oboInOwl:id>
        <rdfs:label>Vodni nadrz Nove Mlyny I</rdfs:label>
    </owl:NamedIndividual>
    


    <!-- http://purl.obolibrary.org/obo/GAZ_00467243 -->

    <owl:NamedIndividual rdf:about="http://purl.obolibrary.org/obo/GAZ_00467243">
        <obo:IAO_0000115>A resevoir.</obo:IAO_0000115>
        <oboInOwl:hasOBONamespace>GAZ</oboInOwl:hasOBONamespace>
        <oboInOwl:id>GAZ:00467243</oboInOwl:id>
        <rdfs:label>Vodni nadrz Brezova</rdfs:label>
    </owl:NamedIndividual>
    


    <!-- http://purl.obolibrary.org/obo/GAZ_00467247 -->

    <owl:NamedIndividual rdf:about="http://purl.obolibrary.org/obo/GAZ_00467247">
        <obo:IAO_0000115>A reservoir.</obo:IAO_0000115>
        <oboInOwl:hasOBONamespace>GAZ</oboInOwl:hasOBONamespace>
        <oboInOwl:id>GAZ:00467247</oboInOwl:id>
        <rdfs:label>Vodni nadrz Horka</rdfs:label>
    </owl:NamedIndividual>
    


    <!-- http://purl.obolibrary.org/obo/GAZ_00467252 -->

    <owl:NamedIndividual rdf:about="http://purl.obolibrary.org/obo/GAZ_00467252">
        <obo:RO_0001025 rdf:resource="http://purl.obolibrary.org/obo/GAZ_00148561"/>
        <obo:IAO_0000115>A reservoir.</obo:IAO_0000115>
        <oboInOwl:hasOBONamespace>GAZ</oboInOwl:hasOBONamespace>
        <oboInOwl:id>GAZ:00467252</oboInOwl:id>
        <rdfs:label>Vodni nadrz Jesenice</rdfs:label>
    </owl:NamedIndividual>
    


    <!-- http://purl.obolibrary.org/obo/GAZ_00467292 -->

    <owl:NamedIndividual rdf:about="http://purl.obolibrary.org/obo/GAZ_00467292">
        <obo:IAO_0000115>A reservoir.</obo:IAO_0000115>
        <oboInOwl:hasOBONamespace>GAZ</oboInOwl:hasOBONamespace>
        <oboInOwl:id>GAZ:00467292</oboInOwl:id>
        <rdfs:label>Vodni nadrz Podhora</rdfs:label>
    </owl:NamedIndividual>
    


    <!-- http://purl.obolibrary.org/obo/GAZ_00467293 -->

    <owl:NamedIndividual rdf:about="http://purl.obolibrary.org/obo/GAZ_00467293">
        <obo:IAO_0000115>A reservoir.</obo:IAO_0000115>
        <oboInOwl:hasOBONamespace>GAZ</oboInOwl:hasOBONamespace>
        <oboInOwl:id>GAZ:00467293</oboInOwl:id>
        <rdfs:label>Vodni nadrz Stanovice</rdfs:label>
    </owl:NamedIndividual>
    


    <!-- http://purl.obolibrary.org/obo/GAZ_00467326 -->

    <owl:NamedIndividual rdf:about="http://purl.obolibrary.org/obo/GAZ_00467326">
        <obo:IAO_0000115>A reservoir.</obo:IAO_0000115>
        <oboInOwl:hasOBONamespace>GAZ</oboInOwl:hasOBONamespace>
        <oboInOwl:id>GAZ:00467326</oboInOwl:id>
        <rdfs:label>Vodni nadrz Baska</rdfs:label>
    </owl:NamedIndividual>
    


    <!-- http://purl.obolibrary.org/obo/GAZ_00467328 -->

    <owl:NamedIndividual rdf:about="http://purl.obolibrary.org/obo/GAZ_00467328">
        <obo:IAO_0000115>A reservoir.</obo:IAO_0000115>
        <oboInOwl:hasOBONamespace>GAZ</oboInOwl:hasOBONamespace>
        <oboInOwl:id>GAZ:00467328</oboInOwl:id>
        <rdfs:label>Vodni nadrz Olesna</rdfs:label>
    </owl:NamedIndividual>
    


    <!-- http://purl.obolibrary.org/obo/GAZ_00467345 -->

    <owl:NamedIndividual rdf:about="http://purl.obolibrary.org/obo/GAZ_00467345">
        <obo:IAO_0000115>A reservoir.</obo:IAO_0000115>
        <oboInOwl:hasOBONamespace>GAZ</oboInOwl:hasOBONamespace>
        <oboInOwl:id>GAZ:00467345</oboInOwl:id>
        <rdfs:label>Vodni nadrz Slezska Harta</rdfs:label>
    </owl:NamedIndividual>
    


    <!-- http://purl.obolibrary.org/obo/GAZ_00467377 -->

    <owl:NamedIndividual rdf:about="http://purl.obolibrary.org/obo/GAZ_00467377">
        <obo:IAO_0000115>A river.</obo:IAO_0000115>
        <oboInOwl:hasOBONamespace>GAZ</oboInOwl:hasOBONamespace>
        <oboInOwl:id>GAZ:00467377</oboInOwl:id>
        <rdfs:label>Hloucela</rdfs:label>
    </owl:NamedIndividual>
    


    <!-- http://purl.obolibrary.org/obo/GAZ_00467378 -->

    <owl:NamedIndividual rdf:about="http://purl.obolibrary.org/obo/GAZ_00467378">
        <obo:RO_0001025 rdf:resource="http://purl.obolibrary.org/obo/GAZ_00467377"/>
        <obo:IAO_0000115>A reservoir.</obo:IAO_0000115>
        <oboInOwl:hasOBONamespace>GAZ</oboInOwl:hasOBONamespace>
        <oboInOwl:id>GAZ:00467378</oboInOwl:id>
        <rdfs:label>Vodni nadrz Plumlov</rdfs:label>
    </owl:NamedIndividual>
    


    <!-- http://purl.obolibrary.org/obo/GAZ_00467500 -->

    <owl:NamedIndividual rdf:about="http://purl.obolibrary.org/obo/GAZ_00467500">
        <obo:IAO_0000115>A reservoir.</obo:IAO_0000115>
        <oboInOwl:hasOBONamespace>GAZ</oboInOwl:hasOBONamespace>
        <oboInOwl:id>GAZ:00467500</oboInOwl:id>
        <rdfs:label>Vodni nadrz Mohelno</rdfs:label>
    </owl:NamedIndividual>
    


    <!-- http://purl.obolibrary.org/obo/GAZ_00467501 -->

    <owl:NamedIndividual rdf:about="http://purl.obolibrary.org/obo/GAZ_00467501">
        <obo:IAO_0000115>A reservoir.</obo:IAO_0000115>
        <oboInOwl:hasOBONamespace>GAZ</oboInOwl:hasOBONamespace>
        <oboInOwl:id>GAZ:00467501</oboInOwl:id>
        <rdfs:label>Vodni nadrz Mostiste</rdfs:label>
    </owl:NamedIndividual>
    


    <!-- http://purl.obolibrary.org/obo/GAZ_00467655 -->

    <owl:NamedIndividual rdf:about="http://purl.obolibrary.org/obo/GAZ_00467655">
        <obo:IAO_0000115>A reservoir.</obo:IAO_0000115>
        <oboInOwl:hasOBONamespace>GAZ</oboInOwl:hasOBONamespace>
        <oboInOwl:id>GAZ:00467655</oboInOwl:id>
        <rdfs:label>Vodni nadrz Vir I</rdfs:label>
    </owl:NamedIndividual>
    


    <!-- http://purl.obolibrary.org/obo/GAZ_00467656 -->

    <owl:NamedIndividual rdf:about="http://purl.obolibrary.org/obo/GAZ_00467656">
        <obo:IAO_0000115>A reservoir.</obo:IAO_0000115>
        <oboInOwl:hasOBONamespace>GAZ</oboInOwl:hasOBONamespace>
        <oboInOwl:id>GAZ:00467656</oboInOwl:id>
        <rdfs:label>Vodni nadrz Vir II</rdfs:label>
    </owl:NamedIndividual>
    


    <!-- http://purl.obolibrary.org/obo/GAZ_00467657 -->

    <owl:NamedIndividual rdf:about="http://purl.obolibrary.org/obo/GAZ_00467657">
        <obo:IAO_0000115>A dam.</obo:IAO_0000115>
        <oboInOwl:hasOBONamespace>GAZ</oboInOwl:hasOBONamespace>
        <oboInOwl:id>GAZ:00467657</oboInOwl:id>
        <rdfs:label>Vir II prehrada</rdfs:label>
    </owl:NamedIndividual>
    


    <!-- http://purl.obolibrary.org/obo/GAZ_00467665 -->

    <owl:NamedIndividual rdf:about="http://purl.obolibrary.org/obo/GAZ_00467665">
        <obo:IAO_0000115>A reservoir.</obo:IAO_0000115>
        <oboInOwl:hasOBONamespace>GAZ</oboInOwl:hasOBONamespace>
        <oboInOwl:id>GAZ:00467665</oboInOwl:id>
        <rdfs:label>Vodni nadrz Korycany</rdfs:label>
    </owl:NamedIndividual>
    


    <!-- http://purl.obolibrary.org/obo/GAZ_00467673 -->

    <owl:NamedIndividual rdf:about="http://purl.obolibrary.org/obo/GAZ_00467673">
        <obo:IAO_0000115>A dam.</obo:IAO_0000115>
        <oboInOwl:hasOBONamespace>GAZ</oboInOwl:hasOBONamespace>
        <oboInOwl:id>GAZ:00467673</oboInOwl:id>
        <rdfs:label>Luhacovicka prehrada</rdfs:label>
    </owl:NamedIndividual>
    


    <!-- http://purl.obolibrary.org/obo/GAZ_00467674 -->

    <owl:NamedIndividual rdf:about="http://purl.obolibrary.org/obo/GAZ_00467674">
        <obo:IAO_0000115>A reservoir.</obo:IAO_0000115>
        <oboInOwl:hasOBONamespace>GAZ</oboInOwl:hasOBONamespace>
        <oboInOwl:id>GAZ:00467674</oboInOwl:id>
        <rdfs:label>Vodni nadrz Ludkovice</rdfs:label>
    </owl:NamedIndividual>
    


    <!-- http://purl.obolibrary.org/obo/GAZ_00467675 -->

    <owl:NamedIndividual rdf:about="http://purl.obolibrary.org/obo/GAZ_00467675">
        <obo:IAO_0000115>A dam.</obo:IAO_0000115>
        <oboInOwl:hasOBONamespace>GAZ</oboInOwl:hasOBONamespace>
        <oboInOwl:id>GAZ:00467675</oboInOwl:id>
        <rdfs:label>Ludkovicka prehrada</rdfs:label>
    </owl:NamedIndividual>
    


    <!-- http://purl.obolibrary.org/obo/GAZ_00467686 -->

    <owl:NamedIndividual rdf:about="http://purl.obolibrary.org/obo/GAZ_00467686">
        <obo:RO_0001025 rdf:resource="http://purl.obolibrary.org/obo/GAZ_00148563"/>
        <obo:IAO_0000115>A reservoir.</obo:IAO_0000115>
        <oboInOwl:hasOBONamespace>GAZ</oboInOwl:hasOBONamespace>
        <oboInOwl:id>GAZ:00467686</oboInOwl:id>
        <rdfs:label>Vodni nadrz Nechranice</rdfs:label>
    </owl:NamedIndividual>
    


    <!-- http://purl.obolibrary.org/obo/GAZ_00467697 -->

    <owl:NamedIndividual rdf:about="http://purl.obolibrary.org/obo/GAZ_00467697">
        <obo:IAO_0000115>A lake.</obo:IAO_0000115>
        <oboInOwl:hasOBONamespace>GAZ</oboInOwl:hasOBONamespace>
        <oboInOwl:id>GAZ:00467697</oboInOwl:id>
        <rdfs:label>Pilsky rybnicek</rdfs:label>
    </owl:NamedIndividual>
    


    <!-- http://purl.obolibrary.org/obo/GAZ_00467952 -->

    <owl:NamedIndividual rdf:about="http://purl.obolibrary.org/obo/GAZ_00467952">
        <obo:IAO_0000115>A lake.</obo:IAO_0000115>
        <oboInOwl:hasOBONamespace>GAZ</oboInOwl:hasOBONamespace>
        <oboInOwl:id>GAZ:00467952</oboInOwl:id>
        <rdfs:label>Kladsky rybnik</rdfs:label>
    </owl:NamedIndividual>
    


    <!-- http://purl.obolibrary.org/obo/GAZ_00468872 -->

    <owl:NamedIndividual rdf:about="http://purl.obolibrary.org/obo/GAZ_00468872">
        <obo:IAO_0000115>A lake.</obo:IAO_0000115>
        <oboInOwl:hasOBONamespace>GAZ</oboInOwl:hasOBONamespace>
        <oboInOwl:id>GAZ:00468872</oboInOwl:id>
        <rdfs:label>Maly Troubny rybnik</rdfs:label>
    </owl:NamedIndividual>
    


    <!-- http://purl.obolibrary.org/obo/GAZ_00468873 -->

    <owl:NamedIndividual rdf:about="http://purl.obolibrary.org/obo/GAZ_00468873">
        <obo:IAO_0000115>A lake.</obo:IAO_0000115>
        <oboInOwl:hasOBONamespace>GAZ</oboInOwl:hasOBONamespace>
        <oboInOwl:id>GAZ:00468873</oboInOwl:id>
        <rdfs:label>Horni Satlava rybnik</rdfs:label>
    </owl:NamedIndividual>
    


    <!-- http://purl.obolibrary.org/obo/GAZ_00468874 -->

    <owl:NamedIndividual rdf:about="http://purl.obolibrary.org/obo/GAZ_00468874">
        <obo:IAO_0000115>A lake.</obo:IAO_0000115>
        <oboInOwl:hasOBONamespace>GAZ</oboInOwl:hasOBONamespace>
        <oboInOwl:id>GAZ:00468874</oboInOwl:id>
        <rdfs:label>Dolni Satlava rybnik</rdfs:label>
    </owl:NamedIndividual>
    


    <!-- http://purl.obolibrary.org/obo/GAZ_00468875 -->

    <owl:NamedIndividual rdf:about="http://purl.obolibrary.org/obo/GAZ_00468875">
        <obo:IAO_0000115>A lake.</obo:IAO_0000115>
        <oboInOwl:hasOBONamespace>GAZ</oboInOwl:hasOBONamespace>
        <oboInOwl:id>GAZ:00468875</oboInOwl:id>
        <rdfs:label>Vozraly rybnik</rdfs:label>
    </owl:NamedIndividual>
    


    <!-- http://purl.obolibrary.org/obo/GAZ_00468876 -->

    <owl:NamedIndividual rdf:about="http://purl.obolibrary.org/obo/GAZ_00468876">
        <obo:IAO_0000115>A lake.</obo:IAO_0000115>
        <oboInOwl:hasOBONamespace>GAZ</oboInOwl:hasOBONamespace>
        <oboInOwl:id>GAZ:00468876</oboInOwl:id>
        <rdfs:label>Stary rybnik</rdfs:label>
    </owl:NamedIndividual>
    


    <!-- http://purl.obolibrary.org/obo/GAZ_00468877 -->

    <owl:NamedIndividual rdf:about="http://purl.obolibrary.org/obo/GAZ_00468877">
        <obo:IAO_0000115>A lake.</obo:IAO_0000115>
        <oboInOwl:hasOBONamespace>GAZ</oboInOwl:hasOBONamespace>
        <oboInOwl:id>GAZ:00468877</oboInOwl:id>
        <rdfs:label>Protrzeny rybnik</rdfs:label>
    </owl:NamedIndividual>
    


    <!-- http://purl.obolibrary.org/obo/GAZ_00468878 -->

    <owl:NamedIndividual rdf:about="http://purl.obolibrary.org/obo/GAZ_00468878">
        <obo:IAO_0000115>A lake.</obo:IAO_0000115>
        <oboInOwl:hasOBONamespace>GAZ</oboInOwl:hasOBONamespace>
        <oboInOwl:id>GAZ:00468878</oboInOwl:id>
        <rdfs:label>Silnicni rybnik</rdfs:label>
    </owl:NamedIndividual>
    


    <!-- http://purl.obolibrary.org/obo/GAZ_00468879 -->

    <owl:NamedIndividual rdf:about="http://purl.obolibrary.org/obo/GAZ_00468879">
        <obo:IAO_0000115>A lake.</obo:IAO_0000115>
        <oboInOwl:hasOBONamespace>GAZ</oboInOwl:hasOBONamespace>
        <oboInOwl:id>GAZ:00468879</oboInOwl:id>
        <rdfs:label>Bejckuv rybnik</rdfs:label>
    </owl:NamedIndividual>
    


    <!-- http://purl.obolibrary.org/obo/GAZ_00469655 -->

    <owl:NamedIndividual rdf:about="http://purl.obolibrary.org/obo/GAZ_00469655">
        <obo:IAO_0000115>A lake.</obo:IAO_0000115>
        <oboInOwl:hasOBONamespace>GAZ</oboInOwl:hasOBONamespace>
        <oboInOwl:id>GAZ:00469655</oboInOwl:id>
        <rdfs:label>Zamis</rdfs:label>
    </owl:NamedIndividual>
    


    <!-- http://purl.obolibrary.org/obo/GAZ_00469656 -->

    <owl:NamedIndividual rdf:about="http://purl.obolibrary.org/obo/GAZ_00469656">
        <obo:IAO_0000115>A lake.</obo:IAO_0000115>
        <oboInOwl:hasOBONamespace>GAZ</oboInOwl:hasOBONamespace>
        <oboInOwl:id>GAZ:00469656</oboInOwl:id>
        <rdfs:label>Tynsky</rdfs:label>
    </owl:NamedIndividual>
    


    <!-- http://purl.obolibrary.org/obo/GAZ_00469657 -->

    <owl:NamedIndividual rdf:about="http://purl.obolibrary.org/obo/GAZ_00469657">
        <obo:IAO_0000115>A lake.</obo:IAO_0000115>
        <oboInOwl:hasOBONamespace>GAZ</oboInOwl:hasOBONamespace>
        <oboInOwl:id>GAZ:00469657</oboInOwl:id>
        <rdfs:label>Hladovy</rdfs:label>
    </owl:NamedIndividual>
    


    <!-- http://purl.obolibrary.org/obo/GAZ_00469658 -->

    <owl:NamedIndividual rdf:about="http://purl.obolibrary.org/obo/GAZ_00469658">
        <obo:IAO_0000115>A lake.</obo:IAO_0000115>
        <oboInOwl:hasOBONamespace>GAZ</oboInOwl:hasOBONamespace>
        <oboInOwl:id>GAZ:00469658</oboInOwl:id>
        <rdfs:label>Barak</rdfs:label>
    </owl:NamedIndividual>
    


    <!-- http://purl.obolibrary.org/obo/GAZ_00469659 -->

    <owl:NamedIndividual rdf:about="http://purl.obolibrary.org/obo/GAZ_00469659">
        <obo:IAO_0000115>A lake.</obo:IAO_0000115>
        <oboInOwl:hasOBONamespace>GAZ</oboInOwl:hasOBONamespace>
        <oboInOwl:id>GAZ:00469659</oboInOwl:id>
        <rdfs:label>Nadymacek</rdfs:label>
    </owl:NamedIndividual>
    


    <!-- http://purl.obolibrary.org/obo/GAZ_00469660 -->

    <owl:NamedIndividual rdf:about="http://purl.obolibrary.org/obo/GAZ_00469660">
        <obo:IAO_0000115>A lake.</obo:IAO_0000115>
        <oboInOwl:hasOBONamespace>GAZ</oboInOwl:hasOBONamespace>
        <oboInOwl:id>GAZ:00469660</oboInOwl:id>
        <rdfs:label>Vodovodni</rdfs:label>
    </owl:NamedIndividual>
    


    <!-- http://purl.obolibrary.org/obo/GAZ_00469661 -->

    <owl:NamedIndividual rdf:about="http://purl.obolibrary.org/obo/GAZ_00469661">
        <obo:IAO_0000115>A lake.</obo:IAO_0000115>
        <oboInOwl:hasOBONamespace>GAZ</oboInOwl:hasOBONamespace>
        <oboInOwl:id>GAZ:00469661</oboInOwl:id>
        <rdfs:label>Baba</rdfs:label>
    </owl:NamedIndividual>
    


    <!-- http://purl.obolibrary.org/obo/GAZ_00469662 -->

    <owl:NamedIndividual rdf:about="http://purl.obolibrary.org/obo/GAZ_00469662">
        <obo:IAO_0000115>A lake.</obo:IAO_0000115>
        <oboInOwl:hasOBONamespace>GAZ</oboInOwl:hasOBONamespace>
        <oboInOwl:id>GAZ:00469662</oboInOwl:id>
        <rdfs:label>Kuchynka</rdfs:label>
    </owl:NamedIndividual>
    


    <!-- http://purl.obolibrary.org/obo/GAZ_00469861 -->

    <owl:NamedIndividual rdf:about="http://purl.obolibrary.org/obo/GAZ_00469861">
        <obo:RO_0001025 rdf:resource="http://purl.obolibrary.org/obo/GAZ_00179205"/>
        <obo:IAO_0000115>A protected area.</obo:IAO_0000115>
        <oboInOwl:hasOBONamespace>GAZ</oboInOwl:hasOBONamespace>
        <oboInOwl:id>GAZ:00469861</oboInOwl:id>
        <rdfs:label>Prirodni rezervace Bile potoky</rdfs:label>
    </owl:NamedIndividual>
    


    <!-- http://purl.obolibrary.org/obo/GAZ_00469862 -->

    <owl:NamedIndividual rdf:about="http://purl.obolibrary.org/obo/GAZ_00469862">
        <obo:RO_0001025 rdf:resource="http://purl.obolibrary.org/obo/GAZ_00179205"/>
        <obo:IAO_0000115>A protected area.</obo:IAO_0000115>
        <oboInOwl:hasOBONamespace>GAZ</oboInOwl:hasOBONamespace>
        <oboInOwl:id>GAZ:00469862</oboInOwl:id>
        <rdfs:label>Prirodni rezervace Dolnonemcanske louky</rdfs:label>
    </owl:NamedIndividual>
    


    <!-- http://purl.obolibrary.org/obo/GAZ_00469863 -->

    <owl:NamedIndividual rdf:about="http://purl.obolibrary.org/obo/GAZ_00469863">
        <obo:RO_0001025 rdf:resource="http://purl.obolibrary.org/obo/GAZ_00179205"/>
        <obo:IAO_0000115>A protected area.</obo:IAO_0000115>
        <oboInOwl:hasOBONamespace>GAZ</oboInOwl:hasOBONamespace>
        <oboInOwl:id>GAZ:00469863</oboInOwl:id>
        <rdfs:label>Prirodni rezervace Drahy</rdfs:label>
    </owl:NamedIndividual>
    


    <!-- http://purl.obolibrary.org/obo/GAZ_00469864 -->

    <owl:NamedIndividual rdf:about="http://purl.obolibrary.org/obo/GAZ_00469864">
        <obo:RO_0001025 rdf:resource="http://purl.obolibrary.org/obo/GAZ_00179205"/>
        <obo:IAO_0000115>A protected area.</obo:IAO_0000115>
        <oboInOwl:hasOBONamespace>GAZ</oboInOwl:hasOBONamespace>
        <oboInOwl:id>GAZ:00469864</oboInOwl:id>
        <rdfs:label>Prirodni rezervace Horni louky</rdfs:label>
    </owl:NamedIndividual>
    


    <!-- http://purl.obolibrary.org/obo/GAZ_00469865 -->

    <owl:NamedIndividual rdf:about="http://purl.obolibrary.org/obo/GAZ_00469865">
        <obo:RO_0001025 rdf:resource="http://purl.obolibrary.org/obo/GAZ_00179205"/>
        <obo:IAO_0000115>A protected area.</obo:IAO_0000115>
        <oboInOwl:hasOBONamespace>GAZ</oboInOwl:hasOBONamespace>
        <oboInOwl:id>GAZ:00469865</oboInOwl:id>
        <rdfs:label>Prirodni rezervace Hute</rdfs:label>
    </owl:NamedIndividual>
    


    <!-- http://purl.obolibrary.org/obo/GAZ_00469866 -->

    <owl:NamedIndividual rdf:about="http://purl.obolibrary.org/obo/GAZ_00469866">
        <obo:RO_0001025 rdf:resource="http://purl.obolibrary.org/obo/GAZ_00179205"/>
        <obo:IAO_0000115>A protected area.</obo:IAO_0000115>
        <oboInOwl:hasOBONamespace>GAZ</oboInOwl:hasOBONamespace>
        <oboInOwl:id>GAZ:00469866</oboInOwl:id>
        <rdfs:label>Prirodni rezervace Jalovcova stran</rdfs:label>
    </owl:NamedIndividual>
    


    <!-- http://purl.obolibrary.org/obo/GAZ_00469867 -->

    <owl:NamedIndividual rdf:about="http://purl.obolibrary.org/obo/GAZ_00469867">
        <obo:RO_0001025 rdf:resource="http://purl.obolibrary.org/obo/GAZ_00179205"/>
        <obo:IAO_0000115>A protected area.</obo:IAO_0000115>
        <oboInOwl:hasOBONamespace>GAZ</oboInOwl:hasOBONamespace>
        <oboInOwl:id>GAZ:00469867</oboInOwl:id>
        <rdfs:label>Prirodni rezervace Javoruvky</rdfs:label>
    </owl:NamedIndividual>
    


    <!-- http://purl.obolibrary.org/obo/GAZ_00469868 -->

    <owl:NamedIndividual rdf:about="http://purl.obolibrary.org/obo/GAZ_00469868">
        <obo:RO_0001025 rdf:resource="http://purl.obolibrary.org/obo/GAZ_00179205"/>
        <obo:IAO_0000115>A protected area.</obo:IAO_0000115>
        <oboInOwl:hasOBONamespace>GAZ</oboInOwl:hasOBONamespace>
        <oboInOwl:id>GAZ:00469868</oboInOwl:id>
        <rdfs:label>Prirodni rezervace Kutky</rdfs:label>
    </owl:NamedIndividual>
    


    <!-- http://purl.obolibrary.org/obo/GAZ_00469869 -->

    <owl:NamedIndividual rdf:about="http://purl.obolibrary.org/obo/GAZ_00469869">
        <obo:RO_0001025 rdf:resource="http://purl.obolibrary.org/obo/GAZ_00179205"/>
        <obo:IAO_0000115>A protected area.</obo:IAO_0000115>
        <oboInOwl:hasOBONamespace>GAZ</oboInOwl:hasOBONamespace>
        <oboInOwl:id>GAZ:00469869</oboInOwl:id>
        <rdfs:label>Prirodni rezervace Lazy</rdfs:label>
    </owl:NamedIndividual>
    


    <!-- http://purl.obolibrary.org/obo/GAZ_00469870 -->

    <owl:NamedIndividual rdf:about="http://purl.obolibrary.org/obo/GAZ_00469870">
        <obo:RO_0001025 rdf:resource="http://purl.obolibrary.org/obo/GAZ_00179205"/>
        <obo:IAO_0000115>A protected area.</obo:IAO_0000115>
        <oboInOwl:hasOBONamespace>GAZ</oboInOwl:hasOBONamespace>
        <oboInOwl:id>GAZ:00469870</oboInOwl:id>
        <rdfs:label>Prirodni rezervace Machova</rdfs:label>
    </owl:NamedIndividual>
    


    <!-- http://purl.obolibrary.org/obo/GAZ_00469871 -->

    <owl:NamedIndividual rdf:about="http://purl.obolibrary.org/obo/GAZ_00469871">
        <obo:RO_0001025 rdf:resource="http://purl.obolibrary.org/obo/GAZ_00179205"/>
        <obo:IAO_0000115>A protected area.</obo:IAO_0000115>
        <oboInOwl:hasOBONamespace>GAZ</oboInOwl:hasOBONamespace>
        <oboInOwl:id>GAZ:00469871</oboInOwl:id>
        <rdfs:label>Prirodni rezervace Nova hora</rdfs:label>
    </owl:NamedIndividual>
    


    <!-- http://purl.obolibrary.org/obo/GAZ_00469872 -->

    <owl:NamedIndividual rdf:about="http://purl.obolibrary.org/obo/GAZ_00469872">
        <obo:RO_0001025 rdf:resource="http://purl.obolibrary.org/obo/GAZ_00179205"/>
        <obo:IAO_0000115>A protected area.</obo:IAO_0000115>
        <oboInOwl:hasOBONamespace>GAZ</oboInOwl:hasOBONamespace>
        <oboInOwl:id>GAZ:00469872</oboInOwl:id>
        <rdfs:label>Prirodni rezervace Plosciny</rdfs:label>
    </owl:NamedIndividual>
    


    <!-- http://purl.obolibrary.org/obo/GAZ_00469873 -->

    <owl:NamedIndividual rdf:about="http://purl.obolibrary.org/obo/GAZ_00469873">
        <obo:RO_0001025 rdf:resource="http://purl.obolibrary.org/obo/GAZ_00179205"/>
        <obo:IAO_0000115>A protected area.</obo:IAO_0000115>
        <oboInOwl:hasOBONamespace>GAZ</oboInOwl:hasOBONamespace>
        <oboInOwl:id>GAZ:00469873</oboInOwl:id>
        <rdfs:label>Prirodni rezervace Pod Zitkovskym vrchem</rdfs:label>
    </owl:NamedIndividual>
    


    <!-- http://purl.obolibrary.org/obo/GAZ_00469874 -->

    <owl:NamedIndividual rdf:about="http://purl.obolibrary.org/obo/GAZ_00469874">
        <obo:RO_0001025 rdf:resource="http://purl.obolibrary.org/obo/GAZ_00179205"/>
        <obo:IAO_0000115>A protected area.</obo:IAO_0000115>
        <oboInOwl:hasOBONamespace>GAZ</oboInOwl:hasOBONamespace>
        <oboInOwl:id>GAZ:00469874</oboInOwl:id>
        <rdfs:label>Prirodni rezervace Sidonie</rdfs:label>
    </owl:NamedIndividual>
    


    <!-- http://purl.obolibrary.org/obo/GAZ_00469875 -->

    <owl:NamedIndividual rdf:about="http://purl.obolibrary.org/obo/GAZ_00469875">
        <obo:RO_0001025 rdf:resource="http://purl.obolibrary.org/obo/GAZ_00179205"/>
        <obo:IAO_0000115>A protected area.</obo:IAO_0000115>
        <oboInOwl:hasOBONamespace>GAZ</oboInOwl:hasOBONamespace>
        <oboInOwl:id>GAZ:00469875</oboInOwl:id>
        <rdfs:label>Prirodni rezervace Ve Vlci</rdfs:label>
    </owl:NamedIndividual>
    


    <!-- http://purl.obolibrary.org/obo/GAZ_00469876 -->

    <owl:NamedIndividual rdf:about="http://purl.obolibrary.org/obo/GAZ_00469876">
        <obo:RO_0001025 rdf:resource="http://purl.obolibrary.org/obo/GAZ_00179205"/>
        <obo:IAO_0000115>A protected area.</obo:IAO_0000115>
        <oboInOwl:hasOBONamespace>GAZ</oboInOwl:hasOBONamespace>
        <oboInOwl:id>GAZ:00469876</oboInOwl:id>
        <rdfs:label>Prirodni pamatka Bahulske jamy</rdfs:label>
    </owl:NamedIndividual>
    


    <!-- http://purl.obolibrary.org/obo/GAZ_00469877 -->

    <owl:NamedIndividual rdf:about="http://purl.obolibrary.org/obo/GAZ_00469877">
        <obo:RO_0001025 rdf:resource="http://purl.obolibrary.org/obo/GAZ_00179205"/>
        <obo:IAO_0000115>A protected area.</obo:IAO_0000115>
        <oboInOwl:hasOBONamespace>GAZ</oboInOwl:hasOBONamespace>
        <oboInOwl:id>GAZ:00469877</oboInOwl:id>
        <rdfs:label>Prirodni pamatka Cestiska</rdfs:label>
    </owl:NamedIndividual>
    


    <!-- http://purl.obolibrary.org/obo/GAZ_00469878 -->

    <owl:NamedIndividual rdf:about="http://purl.obolibrary.org/obo/GAZ_00469878">
        <obo:RO_0001025 rdf:resource="http://purl.obolibrary.org/obo/GAZ_00179205"/>
        <obo:IAO_0000115>A protected area.</obo:IAO_0000115>
        <oboInOwl:hasOBONamespace>GAZ</oboInOwl:hasOBONamespace>
        <oboInOwl:id>GAZ:00469878</oboInOwl:id>
        <rdfs:label>Prirodni pamatka Dobsena</rdfs:label>
    </owl:NamedIndividual>
    


    <!-- http://purl.obolibrary.org/obo/GAZ_00469879 -->

    <owl:NamedIndividual rdf:about="http://purl.obolibrary.org/obo/GAZ_00469879">
        <obo:RO_0001025 rdf:resource="http://purl.obolibrary.org/obo/GAZ_00179205"/>
        <obo:IAO_0000115>A protected area.</obo:IAO_0000115>
        <oboInOwl:hasOBONamespace>GAZ</oboInOwl:hasOBONamespace>
        <oboInOwl:id>GAZ:00469879</oboInOwl:id>
        <rdfs:label>Prirodni pamatka Grun</rdfs:label>
    </owl:NamedIndividual>
    


    <!-- http://purl.obolibrary.org/obo/GAZ_00469880 -->

    <owl:NamedIndividual rdf:about="http://purl.obolibrary.org/obo/GAZ_00469880">
        <obo:RO_0001025 rdf:resource="http://purl.obolibrary.org/obo/GAZ_00179205"/>
        <obo:IAO_0000115>A protected area.</obo:IAO_0000115>
        <oboInOwl:hasOBONamespace>GAZ</oboInOwl:hasOBONamespace>
        <oboInOwl:id>GAZ:00469880</oboInOwl:id>
        <rdfs:label>Prirodni pamatka Hluboce</rdfs:label>
    </owl:NamedIndividual>
    


    <!-- http://purl.obolibrary.org/obo/GAZ_00469881 -->

    <owl:NamedIndividual rdf:about="http://purl.obolibrary.org/obo/GAZ_00469881">
        <obo:RO_0001025 rdf:resource="http://purl.obolibrary.org/obo/GAZ_00179205"/>
        <obo:IAO_0000115>A protected area.</obo:IAO_0000115>
        <oboInOwl:hasOBONamespace>GAZ</oboInOwl:hasOBONamespace>
        <oboInOwl:id>GAZ:00469881</oboInOwl:id>
        <rdfs:label>Prirodni pamatka Hrncarky</rdfs:label>
    </owl:NamedIndividual>
    


    <!-- http://purl.obolibrary.org/obo/GAZ_00469882 -->

    <owl:NamedIndividual rdf:about="http://purl.obolibrary.org/obo/GAZ_00469882">
        <obo:RO_0001025 rdf:resource="http://purl.obolibrary.org/obo/GAZ_00179205"/>
        <obo:IAO_0000115>A protected area.</obo:IAO_0000115>
        <oboInOwl:hasOBONamespace>GAZ</oboInOwl:hasOBONamespace>
        <oboInOwl:id>GAZ:00469882</oboInOwl:id>
        <rdfs:label>Prirodni pamatka Chladny vrch</rdfs:label>
    </owl:NamedIndividual>
    


    <!-- http://purl.obolibrary.org/obo/GAZ_00469883 -->

    <owl:NamedIndividual rdf:about="http://purl.obolibrary.org/obo/GAZ_00469883">
        <obo:RO_0001025 rdf:resource="http://purl.obolibrary.org/obo/GAZ_00179205"/>
        <obo:IAO_0000115>A protected area.</obo:IAO_0000115>
        <oboInOwl:hasOBONamespace>GAZ</oboInOwl:hasOBONamespace>
        <oboInOwl:id>GAZ:00469883</oboInOwl:id>
        <rdfs:label>Prirodni pamatka Chmelinec</rdfs:label>
    </owl:NamedIndividual>
    


    <!-- http://purl.obolibrary.org/obo/GAZ_00469884 -->

    <owl:NamedIndividual rdf:about="http://purl.obolibrary.org/obo/GAZ_00469884">
        <obo:RO_0001025 rdf:resource="http://purl.obolibrary.org/obo/GAZ_00179205"/>
        <obo:IAO_0000115>A protected area.</obo:IAO_0000115>
        <oboInOwl:hasOBONamespace>GAZ</oboInOwl:hasOBONamespace>
        <oboInOwl:id>GAZ:00469884</oboInOwl:id>
        <rdfs:label>Prirodni pamatka Kalabova</rdfs:label>
    </owl:NamedIndividual>
    


    <!-- http://purl.obolibrary.org/obo/GAZ_00469885 -->

    <owl:NamedIndividual rdf:about="http://purl.obolibrary.org/obo/GAZ_00469885">
        <obo:RO_0001025 rdf:resource="http://purl.obolibrary.org/obo/GAZ_00179205"/>
        <obo:IAO_0000115>A protected area.</obo:IAO_0000115>
        <oboInOwl:hasOBONamespace>GAZ</oboInOwl:hasOBONamespace>
        <oboInOwl:id>GAZ:00469885</oboInOwl:id>
        <rdfs:label>Prirodni pamatka Kanoury</rdfs:label>
    </owl:NamedIndividual>
    


    <!-- http://purl.obolibrary.org/obo/GAZ_00469886 -->

    <owl:NamedIndividual rdf:about="http://purl.obolibrary.org/obo/GAZ_00469886">
        <obo:RO_0001025 rdf:resource="http://purl.obolibrary.org/obo/GAZ_00179205"/>
        <obo:IAO_0000115>A protected area.</obo:IAO_0000115>
        <oboInOwl:hasOBONamespace>GAZ</oboInOwl:hasOBONamespace>
        <oboInOwl:id>GAZ:00469886</oboInOwl:id>
        <rdfs:label>Prirodni pamatka Lom Rasova</rdfs:label>
    </owl:NamedIndividual>
    


    <!-- http://purl.obolibrary.org/obo/GAZ_00469887 -->

    <owl:NamedIndividual rdf:about="http://purl.obolibrary.org/obo/GAZ_00469887">
        <obo:RO_0001025 rdf:resource="http://purl.obolibrary.org/obo/GAZ_00179205"/>
        <obo:IAO_0000115>A protected area.</obo:IAO_0000115>
        <oboInOwl:hasOBONamespace>GAZ</oboInOwl:hasOBONamespace>
        <oboInOwl:id>GAZ:00469887</oboInOwl:id>
        <rdfs:label>Prirodni pamatka Mechnacky</rdfs:label>
    </owl:NamedIndividual>
    


    <!-- http://purl.obolibrary.org/obo/GAZ_00469888 -->

    <owl:NamedIndividual rdf:about="http://purl.obolibrary.org/obo/GAZ_00469888">
        <obo:RO_0001025 rdf:resource="http://purl.obolibrary.org/obo/GAZ_00179205"/>
        <obo:IAO_0000115>A protected area.</obo:IAO_0000115>
        <oboInOwl:hasOBONamespace>GAZ</oboInOwl:hasOBONamespace>
        <oboInOwl:id>GAZ:00469888</oboInOwl:id>
        <rdfs:label>Prirodni pamatka Nove louky</rdfs:label>
    </owl:NamedIndividual>
    


    <!-- http://purl.obolibrary.org/obo/GAZ_00469889 -->

    <owl:NamedIndividual rdf:about="http://purl.obolibrary.org/obo/GAZ_00469889">
        <obo:RO_0001025 rdf:resource="http://purl.obolibrary.org/obo/GAZ_00179205"/>
        <obo:IAO_0000115>A protected area.</obo:IAO_0000115>
        <oboInOwl:hasOBONamespace>GAZ</oboInOwl:hasOBONamespace>
        <oboInOwl:id>GAZ:00469889</oboInOwl:id>
        <rdfs:label>Prirodni pamatka Okrouhla</rdfs:label>
    </owl:NamedIndividual>
    


    <!-- http://purl.obolibrary.org/obo/GAZ_00469890 -->

    <owl:NamedIndividual rdf:about="http://purl.obolibrary.org/obo/GAZ_00469890">
        <obo:RO_0001025 rdf:resource="http://purl.obolibrary.org/obo/GAZ_00179205"/>
        <obo:IAO_0000115>A protected area.</obo:IAO_0000115>
        <oboInOwl:hasOBONamespace>GAZ</oboInOwl:hasOBONamespace>
        <oboInOwl:id>GAZ:00469890</oboInOwl:id>
        <rdfs:label>Prirodni pamatka Pod Ciganem</rdfs:label>
    </owl:NamedIndividual>
    


    <!-- http://purl.obolibrary.org/obo/GAZ_00469891 -->

    <owl:NamedIndividual rdf:about="http://purl.obolibrary.org/obo/GAZ_00469891">
        <obo:RO_0001025 rdf:resource="http://purl.obolibrary.org/obo/GAZ_00179205"/>
        <obo:IAO_0000115>A protected area.</obo:IAO_0000115>
        <oboInOwl:hasOBONamespace>GAZ</oboInOwl:hasOBONamespace>
        <oboInOwl:id>GAZ:00469891</oboInOwl:id>
        <rdfs:label>Prirodni pamatka Pod Hribovnou</rdfs:label>
    </owl:NamedIndividual>
    


    <!-- http://purl.obolibrary.org/obo/GAZ_00469892 -->

    <owl:NamedIndividual rdf:about="http://purl.obolibrary.org/obo/GAZ_00469892">
        <obo:RO_0001025 rdf:resource="http://purl.obolibrary.org/obo/GAZ_00179205"/>
        <obo:IAO_0000115>A protected area.</obo:IAO_0000115>
        <oboInOwl:hasOBONamespace>GAZ</oboInOwl:hasOBONamespace>
        <oboInOwl:id>GAZ:00469892</oboInOwl:id>
        <rdfs:label>Prirodni pamatka Pod Vrchy</rdfs:label>
    </owl:NamedIndividual>
    


    <!-- http://purl.obolibrary.org/obo/GAZ_00469893 -->

    <owl:NamedIndividual rdf:about="http://purl.obolibrary.org/obo/GAZ_00469893">
        <obo:RO_0001025 rdf:resource="http://purl.obolibrary.org/obo/GAZ_00179205"/>
        <obo:IAO_0000115>A protected area.</obo:IAO_0000115>
        <oboInOwl:hasOBONamespace>GAZ</oboInOwl:hasOBONamespace>
        <oboInOwl:id>GAZ:00469893</oboInOwl:id>
        <rdfs:label>Prirodni pamatka Rubaniska</rdfs:label>
    </owl:NamedIndividual>
    


    <!-- http://purl.obolibrary.org/obo/GAZ_00469894 -->

    <owl:NamedIndividual rdf:about="http://purl.obolibrary.org/obo/GAZ_00469894">
        <obo:RO_0001025 rdf:resource="http://purl.obolibrary.org/obo/GAZ_00179205"/>
        <obo:IAO_0000115>A protected area.</obo:IAO_0000115>
        <oboInOwl:hasOBONamespace>GAZ</oboInOwl:hasOBONamespace>
        <oboInOwl:id>GAZ:00469894</oboInOwl:id>
        <rdfs:label>Prirodni pamatka Svini hnizdo</rdfs:label>
    </owl:NamedIndividual>
    


    <!-- http://purl.obolibrary.org/obo/GAZ_00469895 -->

    <owl:NamedIndividual rdf:about="http://purl.obolibrary.org/obo/GAZ_00469895">
        <obo:RO_0001025 rdf:resource="http://purl.obolibrary.org/obo/GAZ_00179205"/>
        <obo:IAO_0000115>A protected area.</obo:IAO_0000115>
        <oboInOwl:hasOBONamespace>GAZ</oboInOwl:hasOBONamespace>
        <oboInOwl:id>GAZ:00469895</oboInOwl:id>
        <rdfs:label>Prirodni pamatka Sumlatova</rdfs:label>
    </owl:NamedIndividual>
    


    <!-- http://purl.obolibrary.org/obo/GAZ_00469896 -->

    <owl:NamedIndividual rdf:about="http://purl.obolibrary.org/obo/GAZ_00469896">
        <obo:RO_0001025 rdf:resource="http://purl.obolibrary.org/obo/GAZ_00179205"/>
        <obo:IAO_0000115>A protected area.</obo:IAO_0000115>
        <oboInOwl:hasOBONamespace>GAZ</oboInOwl:hasOBONamespace>
        <oboInOwl:id>GAZ:00469896</oboInOwl:id>
        <rdfs:label>Prirodni pamatka U Petruvky</rdfs:label>
    </owl:NamedIndividual>
    


    <!-- http://purl.obolibrary.org/obo/GAZ_00469897 -->

    <owl:NamedIndividual rdf:about="http://purl.obolibrary.org/obo/GAZ_00469897">
        <obo:RO_0001025 rdf:resource="http://purl.obolibrary.org/obo/GAZ_00179205"/>
        <obo:IAO_0000115>A protected area.</obo:IAO_0000115>
        <oboInOwl:hasOBONamespace>GAZ</oboInOwl:hasOBONamespace>
        <oboInOwl:id>GAZ:00469897</oboInOwl:id>
        <rdfs:label>Prirodni pamatka Uvezene</rdfs:label>
    </owl:NamedIndividual>
    


    <!-- http://purl.obolibrary.org/obo/GAZ_00469898 -->

    <owl:NamedIndividual rdf:about="http://purl.obolibrary.org/obo/GAZ_00469898">
        <obo:RO_0001025 rdf:resource="http://purl.obolibrary.org/obo/GAZ_00179205"/>
        <obo:IAO_0000115>A protected area.</obo:IAO_0000115>
        <oboInOwl:hasOBONamespace>GAZ</oboInOwl:hasOBONamespace>
        <oboInOwl:id>GAZ:00469898</oboInOwl:id>
        <rdfs:label>Prirodni pamatka U zvonice</rdfs:label>
    </owl:NamedIndividual>
    


    <!-- http://purl.obolibrary.org/obo/GAZ_00469899 -->

    <owl:NamedIndividual rdf:about="http://purl.obolibrary.org/obo/GAZ_00469899">
        <obo:RO_0001025 rdf:resource="http://purl.obolibrary.org/obo/GAZ_00179205"/>
        <obo:IAO_0000115>A protected area.</obo:IAO_0000115>
        <oboInOwl:hasOBONamespace>GAZ</oboInOwl:hasOBONamespace>
        <oboInOwl:id>GAZ:00469899</oboInOwl:id>
        <rdfs:label>Prirodni pamatka Vapenky</rdfs:label>
    </owl:NamedIndividual>
    


    <!-- http://purl.obolibrary.org/obo/GAZ_00469900 -->

    <owl:NamedIndividual rdf:about="http://purl.obolibrary.org/obo/GAZ_00469900">
        <obo:RO_0001025 rdf:resource="http://purl.obolibrary.org/obo/GAZ_00179205"/>
        <obo:IAO_0000115>A protected area.</obo:IAO_0000115>
        <oboInOwl:hasOBONamespace>GAZ</oboInOwl:hasOBONamespace>
        <oboInOwl:id>GAZ:00469900</oboInOwl:id>
        <rdfs:label>Prirodni pamatka V Kratkych</rdfs:label>
    </owl:NamedIndividual>
    


    <!-- http://purl.obolibrary.org/obo/GAZ_00469901 -->

    <owl:NamedIndividual rdf:about="http://purl.obolibrary.org/obo/GAZ_00469901">
        <obo:RO_0001025 rdf:resource="http://purl.obolibrary.org/obo/GAZ_00179205"/>
        <obo:IAO_0000115>A protected area.</obo:IAO_0000115>
        <oboInOwl:hasOBONamespace>GAZ</oboInOwl:hasOBONamespace>
        <oboInOwl:id>GAZ:00469901</oboInOwl:id>
        <rdfs:label>Prirodni pamatka Zahumenice</rdfs:label>
    </owl:NamedIndividual>
    


    <!-- http://purl.obolibrary.org/obo/GAZ_00469902 -->

    <owl:NamedIndividual rdf:about="http://purl.obolibrary.org/obo/GAZ_00469902">
        <obo:RO_0001025 rdf:resource="http://purl.obolibrary.org/obo/GAZ_00179205"/>
        <obo:IAO_0000115>A protected area.</obo:IAO_0000115>
        <oboInOwl:hasOBONamespace>GAZ</oboInOwl:hasOBONamespace>
        <oboInOwl:id>GAZ:00469902</oboInOwl:id>
        <rdfs:label>Prirodni pamatka Za lesem</rdfs:label>
    </owl:NamedIndividual>
    


    <!-- http://purl.obolibrary.org/obo/GAZ_00469903 -->

    <owl:NamedIndividual rdf:about="http://purl.obolibrary.org/obo/GAZ_00469903">
        <obo:RO_0001025 rdf:resource="http://purl.obolibrary.org/obo/GAZ_00179205"/>
        <obo:IAO_0000115>A protected area.</obo:IAO_0000115>
        <oboInOwl:hasOBONamespace>GAZ</oboInOwl:hasOBONamespace>
        <oboInOwl:id>GAZ:00469903</oboInOwl:id>
        <rdfs:label>Prirodni pamatka Zerotin</rdfs:label>
    </owl:NamedIndividual>
    


    <!-- http://purl.obolibrary.org/obo/GAZ_00469904 -->

    <owl:NamedIndividual rdf:about="http://purl.obolibrary.org/obo/GAZ_00469904">
        <obo:RO_0001025 rdf:resource="http://purl.obolibrary.org/obo/GAZ_00179205"/>
        <obo:IAO_0000115>A protected area.</obo:IAO_0000115>
        <oboInOwl:hasOBONamespace>GAZ</oboInOwl:hasOBONamespace>
        <oboInOwl:id>GAZ:00469904</oboInOwl:id>
        <rdfs:label>Prirodni pamatka Zleb</rdfs:label>
    </owl:NamedIndividual>
    


    <!-- http://purl.obolibrary.org/obo/GAZ_00469967 -->

    <owl:NamedIndividual rdf:about="http://purl.obolibrary.org/obo/GAZ_00469967">
        <obo:RO_0001025 rdf:resource="http://purl.obolibrary.org/obo/GAZ_00465556"/>
        <obo:IAO_0000115>A protected area.</obo:IAO_0000115>
        <oboInOwl:hasOBONamespace>GAZ</oboInOwl:hasOBONamespace>
        <oboInOwl:id>GAZ:00469967</oboInOwl:id>
        <rdfs:label>Prirodni rezervace Bartosovicky luh</rdfs:label>
    </owl:NamedIndividual>
    


    <!-- http://purl.obolibrary.org/obo/GAZ_00469968 -->

    <owl:NamedIndividual rdf:about="http://purl.obolibrary.org/obo/GAZ_00469968">
        <obo:RO_0001025 rdf:resource="http://purl.obolibrary.org/obo/GAZ_00465556"/>
        <obo:IAO_0000115>A protected area.</obo:IAO_0000115>
        <oboInOwl:hasOBONamespace>GAZ</oboInOwl:hasOBONamespace>
        <oboInOwl:id>GAZ:00469968</oboInOwl:id>
        <rdfs:label>Prirodni rezervace Bariny</rdfs:label>
    </owl:NamedIndividual>
    


    <!-- http://purl.obolibrary.org/obo/GAZ_00469969 -->

    <owl:NamedIndividual rdf:about="http://purl.obolibrary.org/obo/GAZ_00469969">
        <obo:RO_0001025 rdf:resource="http://purl.obolibrary.org/obo/GAZ_00465556"/>
        <obo:IAO_0000115>A protected area.</obo:IAO_0000115>
        <oboInOwl:hasOBONamespace>GAZ</oboInOwl:hasOBONamespace>
        <oboInOwl:id>GAZ:00469969</oboInOwl:id>
        <rdfs:label>Prirodni rezervace Bazantula</rdfs:label>
    </owl:NamedIndividual>
    


    <!-- http://purl.obolibrary.org/obo/GAZ_00469970 -->

    <owl:NamedIndividual rdf:about="http://purl.obolibrary.org/obo/GAZ_00469970">
        <obo:RO_0001025 rdf:resource="http://purl.obolibrary.org/obo/GAZ_00465556"/>
        <obo:IAO_0000115>A protected area.</obo:IAO_0000115>
        <oboInOwl:hasOBONamespace>GAZ</oboInOwl:hasOBONamespace>
        <oboInOwl:id>GAZ:00469970</oboInOwl:id>
        <rdfs:label>Prirodni rezervace Koryta</rdfs:label>
    </owl:NamedIndividual>
    


    <!-- http://purl.obolibrary.org/obo/GAZ_00469971 -->

    <owl:NamedIndividual rdf:about="http://purl.obolibrary.org/obo/GAZ_00469971">
        <obo:RO_0001025 rdf:resource="http://purl.obolibrary.org/obo/GAZ_00465556"/>
        <obo:IAO_0000115>A protected area.</obo:IAO_0000115>
        <oboInOwl:hasOBONamespace>GAZ</oboInOwl:hasOBONamespace>
        <oboInOwl:id>GAZ:00469971</oboInOwl:id>
        <rdfs:label>Prirodni rezervace Kotvice</rdfs:label>
    </owl:NamedIndividual>
    


    <!-- http://purl.obolibrary.org/obo/GAZ_00469972 -->

    <owl:NamedIndividual rdf:about="http://purl.obolibrary.org/obo/GAZ_00469972">
        <obo:RO_0001025 rdf:resource="http://purl.obolibrary.org/obo/GAZ_00465556"/>
        <obo:IAO_0000115>A protected area.</obo:IAO_0000115>
        <oboInOwl:hasOBONamespace>GAZ</oboInOwl:hasOBONamespace>
        <oboInOwl:id>GAZ:00469972</oboInOwl:id>
        <rdfs:label>Prirodni rezervace Polansky les</rdfs:label>
    </owl:NamedIndividual>
    


    <!-- http://purl.obolibrary.org/obo/GAZ_00469973 -->

    <owl:NamedIndividual rdf:about="http://purl.obolibrary.org/obo/GAZ_00469973">
        <obo:RO_0001025 rdf:resource="http://purl.obolibrary.org/obo/GAZ_00465556"/>
        <obo:IAO_0000115>A protected area.</obo:IAO_0000115>
        <oboInOwl:hasOBONamespace>GAZ</oboInOwl:hasOBONamespace>
        <oboInOwl:id>GAZ:00469973</oboInOwl:id>
        <rdfs:label>Prirodni rezervace Rakosina</rdfs:label>
    </owl:NamedIndividual>
    


    <!-- http://purl.obolibrary.org/obo/GAZ_00469974 -->

    <owl:NamedIndividual rdf:about="http://purl.obolibrary.org/obo/GAZ_00469974">
        <obo:RO_0001025 rdf:resource="http://purl.obolibrary.org/obo/GAZ_00465556"/>
        <obo:IAO_0000115>A protected area.</obo:IAO_0000115>
        <oboInOwl:hasOBONamespace>GAZ</oboInOwl:hasOBONamespace>
        <oboInOwl:id>GAZ:00469974</oboInOwl:id>
        <rdfs:label>Prirodni pamatka Meandry stare Odry</rdfs:label>
    </owl:NamedIndividual>
    


    <!-- http://purl.obolibrary.org/obo/GAZ_00469975 -->

    <owl:NamedIndividual rdf:about="http://purl.obolibrary.org/obo/GAZ_00469975">
        <obo:RO_0001025 rdf:resource="http://purl.obolibrary.org/obo/GAZ_00465556"/>
        <obo:IAO_0000115>A protected area.</obo:IAO_0000115>
        <oboInOwl:hasOBONamespace>GAZ</oboInOwl:hasOBONamespace>
        <oboInOwl:id>GAZ:00469975</oboInOwl:id>
        <rdfs:label>Prirodni pamatka Puste nivy</rdfs:label>
    </owl:NamedIndividual>
    


    <!-- http://purl.obolibrary.org/obo/GAZ_00469976 -->

    <owl:NamedIndividual rdf:about="http://purl.obolibrary.org/obo/GAZ_00469976">
        <obo:RO_0001025 rdf:resource="http://purl.obolibrary.org/obo/GAZ_00466014"/>
        <obo:IAO_0000115>A protected area.</obo:IAO_0000115>
        <oboInOwl:hasOBONamespace>GAZ</oboInOwl:hasOBONamespace>
        <oboInOwl:id>GAZ:00469976</oboInOwl:id>
        <rdfs:label>Prirodni rezervace Lisci vrch</rdfs:label>
    </owl:NamedIndividual>
    


    <!-- http://purl.obolibrary.org/obo/GAZ_00469977 -->

    <owl:NamedIndividual rdf:about="http://purl.obolibrary.org/obo/GAZ_00469977">
        <obo:RO_0001025 rdf:resource="http://purl.obolibrary.org/obo/GAZ_00466014"/>
        <obo:IAO_0000115>A protected area.</obo:IAO_0000115>
        <oboInOwl:hasOBONamespace>GAZ</oboInOwl:hasOBONamespace>
        <oboInOwl:id>GAZ:00469977</oboInOwl:id>
        <rdfs:label>Prirodni rezervace Milovicka stran</rdfs:label>
    </owl:NamedIndividual>
    


    <!-- http://purl.obolibrary.org/obo/GAZ_00469978 -->

    <owl:NamedIndividual rdf:about="http://purl.obolibrary.org/obo/GAZ_00469978">
        <obo:RO_0001025 rdf:resource="http://purl.obolibrary.org/obo/GAZ_00466014"/>
        <obo:IAO_0000115>A protected area.</obo:IAO_0000115>
        <oboInOwl:hasOBONamespace>GAZ</oboInOwl:hasOBONamespace>
        <oboInOwl:id>GAZ:00469978</oboInOwl:id>
        <rdfs:label>Prirodni rezervace Svaty kopecek</rdfs:label>
    </owl:NamedIndividual>
    


    <!-- http://purl.obolibrary.org/obo/GAZ_00469979 -->

    <owl:NamedIndividual rdf:about="http://purl.obolibrary.org/obo/GAZ_00469979">
        <obo:RO_0001025 rdf:resource="http://purl.obolibrary.org/obo/GAZ_00466014"/>
        <obo:IAO_0000115>A protected area.</obo:IAO_0000115>
        <oboInOwl:hasOBONamespace>GAZ</oboInOwl:hasOBONamespace>
        <oboInOwl:id>GAZ:00469979</oboInOwl:id>
        <rdfs:label>Prirodni rezervace Sibenicnik</rdfs:label>
    </owl:NamedIndividual>
    


    <!-- http://purl.obolibrary.org/obo/GAZ_00469980 -->

    <owl:NamedIndividual rdf:about="http://purl.obolibrary.org/obo/GAZ_00469980">
        <obo:RO_0001025 rdf:resource="http://purl.obolibrary.org/obo/GAZ_00466014"/>
        <obo:IAO_0000115>A protected area.</obo:IAO_0000115>
        <oboInOwl:hasOBONamespace>GAZ</oboInOwl:hasOBONamespace>
        <oboInOwl:id>GAZ:00469980</oboInOwl:id>
        <rdfs:label>Prirodni rezervace Turold</rdfs:label>
    </owl:NamedIndividual>
    


    <!-- http://purl.obolibrary.org/obo/GAZ_00469981 -->

    <owl:NamedIndividual rdf:about="http://purl.obolibrary.org/obo/GAZ_00469981">
        <obo:RO_0001025 rdf:resource="http://purl.obolibrary.org/obo/GAZ_00466014"/>
        <obo:IAO_0000115>A protected area.</obo:IAO_0000115>
        <oboInOwl:hasOBONamespace>GAZ</oboInOwl:hasOBONamespace>
        <oboInOwl:id>GAZ:00469981</oboInOwl:id>
        <rdfs:label>Prirodni pamatka Anensky vrch</rdfs:label>
    </owl:NamedIndividual>
    


    <!-- http://purl.obolibrary.org/obo/GAZ_00469982 -->

    <owl:NamedIndividual rdf:about="http://purl.obolibrary.org/obo/GAZ_00469982">
        <obo:RO_0001025 rdf:resource="http://purl.obolibrary.org/obo/GAZ_00466014"/>
        <obo:IAO_0000115>A protected area.</obo:IAO_0000115>
        <oboInOwl:hasOBONamespace>GAZ</oboInOwl:hasOBONamespace>
        <oboInOwl:id>GAZ:00469982</oboInOwl:id>
        <rdfs:label>Prirodni pamatka Kienberg</rdfs:label>
    </owl:NamedIndividual>
    


    <!-- http://purl.obolibrary.org/obo/GAZ_00469983 -->

    <owl:NamedIndividual rdf:about="http://purl.obolibrary.org/obo/GAZ_00469983">
        <obo:RO_0001025 rdf:resource="http://purl.obolibrary.org/obo/GAZ_00466014"/>
        <obo:IAO_0000115>A protected area.</obo:IAO_0000115>
        <oboInOwl:hasOBONamespace>GAZ</oboInOwl:hasOBONamespace>
        <oboInOwl:id>GAZ:00469983</oboInOwl:id>
        <rdfs:label>Prirodni pamatka Kocici skala</rdfs:label>
    </owl:NamedIndividual>
    


    <!-- http://purl.obolibrary.org/obo/GAZ_00469984 -->

    <owl:NamedIndividual rdf:about="http://purl.obolibrary.org/obo/GAZ_00469984">
        <obo:RO_0001025 rdf:resource="http://purl.obolibrary.org/obo/GAZ_00466014"/>
        <obo:IAO_0000115>A protected area.</obo:IAO_0000115>
        <oboInOwl:hasOBONamespace>GAZ</oboInOwl:hasOBONamespace>
        <oboInOwl:id>GAZ:00469984</oboInOwl:id>
        <rdfs:label>Prirodni pamatka Ruzovy kopec</rdfs:label>
    </owl:NamedIndividual>
    


    <!-- http://purl.obolibrary.org/obo/GAZ_00470821 -->

    <owl:NamedIndividual rdf:about="http://purl.obolibrary.org/obo/GAZ_00470821">
        <obo:IAO_0000115>A river.</obo:IAO_0000115>
        <oboInOwl:hasOBONamespace>GAZ</oboInOwl:hasOBONamespace>
        <oboInOwl:id>GAZ:00470821</oboInOwl:id>
        <rdfs:label>Furcowka</rdfs:label>
    </owl:NamedIndividual>
    


    <!-- http://purl.obolibrary.org/obo/GAZ_00470822 -->

    <owl:NamedIndividual rdf:about="http://purl.obolibrary.org/obo/GAZ_00470822">
        <obo:IAO_0000115>A river.</obo:IAO_0000115>
        <oboInOwl:hasOBONamespace>GAZ</oboInOwl:hasOBONamespace>
        <oboInOwl:id>GAZ:00470822</oboInOwl:id>
        <rdfs:label>Potok Foredowki</rdfs:label>
    </owl:NamedIndividual>
    


    <!-- http://purl.obolibrary.org/obo/GAZ_00470823 -->

    <owl:NamedIndividual rdf:about="http://purl.obolibrary.org/obo/GAZ_00470823">
        <obo:IAO_0000115>A river.</obo:IAO_0000115>
        <oboInOwl:hasOBONamespace>GAZ</oboInOwl:hasOBONamespace>
        <oboInOwl:id>GAZ:00470823</oboInOwl:id>
        <rdfs:label>Jaszcze, Jamne</rdfs:label>
    </owl:NamedIndividual>
    


    <!-- http://purl.obolibrary.org/obo/GAZ_00470824 -->

    <owl:NamedIndividual rdf:about="http://purl.obolibrary.org/obo/GAZ_00470824">
        <obo:IAO_0000115>A river.</obo:IAO_0000115>
        <oboInOwl:hasOBONamespace>GAZ</oboInOwl:hasOBONamespace>
        <oboInOwl:id>GAZ:00470824</oboInOwl:id>
        <rdfs:label>Potok Skrodne</rdfs:label>
    </owl:NamedIndividual>
    


    <!-- http://purl.obolibrary.org/obo/GAZ_00470825 -->

    <owl:NamedIndividual rdf:about="http://purl.obolibrary.org/obo/GAZ_00470825">
        <obo:IAO_0000115>A river.</obo:IAO_0000115>
        <oboInOwl:hasOBONamespace>GAZ</oboInOwl:hasOBONamespace>
        <oboInOwl:id>GAZ:00470825</oboInOwl:id>
        <rdfs:label>Potok Gorcowy</rdfs:label>
    </owl:NamedIndividual>
    


    <!-- http://purl.obolibrary.org/obo/GAZ_00470826 -->

    <owl:NamedIndividual rdf:about="http://purl.obolibrary.org/obo/GAZ_00470826">
        <obo:IAO_0000115>A river.</obo:IAO_0000115>
        <oboInOwl:hasOBONamespace>GAZ</oboInOwl:hasOBONamespace>
        <oboInOwl:id>GAZ:00470826</oboInOwl:id>
        <rdfs:label>Potok Jurkowski</rdfs:label>
    </owl:NamedIndividual>
    


    <!-- http://purl.obolibrary.org/obo/GAZ_00470827 -->

    <owl:NamedIndividual rdf:about="http://purl.obolibrary.org/obo/GAZ_00470827">
        <obo:IAO_0000115>A river.</obo:IAO_0000115>
        <oboInOwl:hasOBONamespace>GAZ</oboInOwl:hasOBONamespace>
        <oboInOwl:id>GAZ:00470827</oboInOwl:id>
        <rdfs:label>Potok Kudowski</rdfs:label>
    </owl:NamedIndividual>
    


    <!-- http://purl.obolibrary.org/obo/GAZ_00470828 -->

    <owl:NamedIndividual rdf:about="http://purl.obolibrary.org/obo/GAZ_00470828">
        <obo:IAO_0000115>A river.</obo:IAO_0000115>
        <oboInOwl:hasOBONamespace>GAZ</oboInOwl:hasOBONamespace>
        <oboInOwl:id>GAZ:00470828</oboInOwl:id>
        <rdfs:label>Szymanowski</rdfs:label>
    </owl:NamedIndividual>
    


    <!-- http://purl.obolibrary.org/obo/GAZ_00470829 -->

    <owl:NamedIndividual rdf:about="http://purl.obolibrary.org/obo/GAZ_00470829">
        <obo:IAO_0000115>A river.</obo:IAO_0000115>
        <oboInOwl:hasOBONamespace>GAZ</oboInOwl:hasOBONamespace>
        <oboInOwl:id>GAZ:00470829</oboInOwl:id>
        <rdfs:label>Potok Lubanski</rdfs:label>
    </owl:NamedIndividual>
    


    <!-- http://purl.obolibrary.org/obo/GAZ_00470830 -->

    <owl:NamedIndividual rdf:about="http://purl.obolibrary.org/obo/GAZ_00470830">
        <obo:IAO_0000115>A river.</obo:IAO_0000115>
        <oboInOwl:hasOBONamespace>GAZ</oboInOwl:hasOBONamespace>
        <oboInOwl:id>GAZ:00470830</oboInOwl:id>
        <rdfs:label>Potok Rolnicki</rdfs:label>
    </owl:NamedIndividual>
    


    <!-- http://purl.obolibrary.org/obo/GAZ_00471814 -->

    <owl:NamedIndividual rdf:about="http://purl.obolibrary.org/obo/GAZ_00471814">
        <obo:RO_0001025 rdf:resource="http://purl.obolibrary.org/obo/GAZ_00061772"/>
        <obo:IAO_0000115>A protected area.</obo:IAO_0000115>
        <oboInOwl:hasOBONamespace>GAZ</oboInOwl:hasOBONamespace>
        <oboInOwl:id>GAZ:00471814</oboInOwl:id>
        <rdfs:label>Rezerwat przyrody Biala Woda</rdfs:label>
    </owl:NamedIndividual>
    


    <!-- http://purl.obolibrary.org/obo/GAZ_00471815 -->

    <owl:NamedIndividual rdf:about="http://purl.obolibrary.org/obo/GAZ_00471815">
        <obo:RO_0001025 rdf:resource="http://purl.obolibrary.org/obo/GAZ_00061772"/>
        <obo:IAO_0000115>A protected area.</obo:IAO_0000115>
        <oboInOwl:hasOBONamespace>GAZ</oboInOwl:hasOBONamespace>
        <oboInOwl:id>GAZ:00471815</oboInOwl:id>
        <rdfs:label>Rezerwat przyrody Przelom Bialki pod Krempachami</rdfs:label>
    </owl:NamedIndividual>
    


    <!-- http://purl.obolibrary.org/obo/GAZ_00471816 -->

    <owl:NamedIndividual rdf:about="http://purl.obolibrary.org/obo/GAZ_00471816">
        <obo:RO_0001025 rdf:resource="http://purl.obolibrary.org/obo/GAZ_00061772"/>
        <obo:IAO_0000115>A protected area.</obo:IAO_0000115>
        <oboInOwl:hasOBONamespace>GAZ</oboInOwl:hasOBONamespace>
        <oboInOwl:id>GAZ:00471816</oboInOwl:id>
        <rdfs:label>Rezerwat przyrody Wawoz Homole</rdfs:label>
    </owl:NamedIndividual>
    


    <!-- http://purl.obolibrary.org/obo/GAZ_00471817 -->

    <owl:NamedIndividual rdf:about="http://purl.obolibrary.org/obo/GAZ_00471817">
        <obo:RO_0001025 rdf:resource="http://purl.obolibrary.org/obo/GAZ_00061772"/>
        <obo:IAO_0000115>A protected area.</obo:IAO_0000115>
        <oboInOwl:hasOBONamespace>GAZ</oboInOwl:hasOBONamespace>
        <oboInOwl:id>GAZ:00471817</oboInOwl:id>
        <rdfs:label>Rezerwat przyrody Wysokie Skalki</rdfs:label>
    </owl:NamedIndividual>
    


    <!-- http://purl.obolibrary.org/obo/GAZ_00471818 -->

    <owl:NamedIndividual rdf:about="http://purl.obolibrary.org/obo/GAZ_00471818">
        <obo:RO_0001025 rdf:resource="http://purl.obolibrary.org/obo/GAZ_00061772"/>
        <obo:IAO_0000115>A protected area.</obo:IAO_0000115>
        <oboInOwl:hasOBONamespace>GAZ</oboInOwl:hasOBONamespace>
        <oboInOwl:id>GAZ:00471818</oboInOwl:id>
        <rdfs:label>Rezerwat przyrody Zaskalskie-Bodnarowka</rdfs:label>
    </owl:NamedIndividual>
    


    <!-- http://purl.obolibrary.org/obo/GAZ_00471825 -->

    <owl:NamedIndividual rdf:about="http://purl.obolibrary.org/obo/GAZ_00471825">
        <obo:RO_0001025 rdf:resource="http://purl.obolibrary.org/obo/GAZ_00061777"/>
        <obo:IAO_0000115>A protected area. Located in the southern part of the country, in Lesser Poland Voivodeship, on the border with Slovakia.</obo:IAO_0000115>
        <oboInOwl:hasOBONamespace>GAZ</oboInOwl:hasOBONamespace>
        <oboInOwl:id>GAZ:00471825</oboInOwl:id>
        <rdfs:label>Babiogorski Park Narodowy</rdfs:label>
    </owl:NamedIndividual>
    


    <!-- http://purl.obolibrary.org/obo/GAZ_00471826 -->

    <owl:NamedIndividual rdf:about="http://purl.obolibrary.org/obo/GAZ_00471826">
        <obo:RO_0001025 rdf:resource="http://purl.obolibrary.org/obo/GAZ_00061763"/>
        <obo:IAO_0000115>A protected area. It covers central and northeastern parts of the Gorce mountains, which are part of the Western Beskids.</obo:IAO_0000115>
        <oboInOwl:hasOBONamespace>GAZ</oboInOwl:hasOBONamespace>
        <oboInOwl:id>GAZ:00471826</oboInOwl:id>
        <rdfs:label>Gorczanski Park Narodowy</rdfs:label>
    </owl:NamedIndividual>
    


    <!-- http://purl.obolibrary.org/obo/GAZ_00471827 -->

    <owl:NamedIndividual rdf:about="http://purl.obolibrary.org/obo/GAZ_00471827">
        <obo:RO_0001025 rdf:resource="http://purl.obolibrary.org/obo/GAZ_00061698"/>
        <obo:IAO_0000115>A geological group of mountain ranges of the Outer Eastern Carpathians, mostly in Ukraine. The region includes the mountainous far southeastern point of Poland and the far eastern point of Slovakia, then stretches southward through western Ukraine to the Romanian border.</obo:IAO_0000115>
        <oboInOwl:hasOBONamespace>GAZ</oboInOwl:hasOBONamespace>
        <oboInOwl:id>GAZ:00471827</oboInOwl:id>
        <rdfs:label>Eastern Beskids and the Ukrainian Carpathians</rdfs:label>
    </owl:NamedIndividual>
    


    <!-- http://purl.obolibrary.org/obo/GAZ_00471829 -->

    <owl:NamedIndividual rdf:about="http://purl.obolibrary.org/obo/GAZ_00471829">
        <obo:RO_0001025 rdf:resource="http://purl.obolibrary.org/obo/GAZ_00061932"/>
        <obo:IAO_0000115>A protected area.</obo:IAO_0000115>
        <oboInOwl:hasOBONamespace>GAZ</oboInOwl:hasOBONamespace>
        <oboInOwl:id>GAZ:00471829</oboInOwl:id>
        <rdfs:label>Magurski Park Narodowy</rdfs:label>
    </owl:NamedIndividual>
    


    <!-- http://purl.obolibrary.org/obo/GAZ_00471830 -->

    <owl:NamedIndividual rdf:about="http://purl.obolibrary.org/obo/GAZ_00471830">
        <obo:RO_0001025 rdf:resource="http://purl.obolibrary.org/obo/GAZ_00061848"/>
        <obo:IAO_0000115>A mountain lake on the Polish side of Mount Rysy in the Tatra mountains.</obo:IAO_0000115>
        <oboInOwl:hasOBONamespace>GAZ</oboInOwl:hasOBONamespace>
        <oboInOwl:id>GAZ:00471830</oboInOwl:id>
        <rdfs:label>Czarny Staw pod Rysami</rdfs:label>
    </owl:NamedIndividual>
    


    <!-- http://purl.obolibrary.org/obo/GAZ_00471831 -->

    <owl:NamedIndividual rdf:about="http://purl.obolibrary.org/obo/GAZ_00471831">
        <obo:RO_0001025 rdf:resource="http://purl.obolibrary.org/obo/GAZ_00481063"/>
        <obo:IAO_0000115>A lake.</obo:IAO_0000115>
        <oboInOwl:hasOBONamespace>GAZ</oboInOwl:hasOBONamespace>
        <oboInOwl:id>GAZ:00471831</oboInOwl:id>
        <rdfs:label>Przedni Staw Polski</rdfs:label>
    </owl:NamedIndividual>
    


    <!-- http://purl.obolibrary.org/obo/GAZ_00471832 -->

    <owl:NamedIndividual rdf:about="http://purl.obolibrary.org/obo/GAZ_00471832">
        <obo:RO_0001025 rdf:resource="http://purl.obolibrary.org/obo/GAZ_00481063"/>
        <obo:IAO_0000115>A lake.</obo:IAO_0000115>
        <oboInOwl:hasOBONamespace>GAZ</oboInOwl:hasOBONamespace>
        <oboInOwl:id>GAZ:00471832</oboInOwl:id>
        <rdfs:label>Maly Staw Polski</rdfs:label>
    </owl:NamedIndividual>
    


    <!-- http://purl.obolibrary.org/obo/GAZ_00471834 -->

    <owl:NamedIndividual rdf:about="http://purl.obolibrary.org/obo/GAZ_00471834">
        <obo:RO_0001025 rdf:resource="http://purl.obolibrary.org/obo/GAZ_00481063"/>
        <obo:IAO_0000115>A lake.</obo:IAO_0000115>
        <oboInOwl:hasOBONamespace>GAZ</oboInOwl:hasOBONamespace>
        <oboInOwl:id>GAZ:00471834</oboInOwl:id>
        <rdfs:label>Zadni Staw Polski</rdfs:label>
    </owl:NamedIndividual>
    


    <!-- http://purl.obolibrary.org/obo/GAZ_00471835 -->

    <owl:NamedIndividual rdf:about="http://purl.obolibrary.org/obo/GAZ_00471835">
        <obo:RO_0001025 rdf:resource="http://purl.obolibrary.org/obo/GAZ_00481063"/>
        <obo:IAO_0000115>A lake.</obo:IAO_0000115>
        <oboInOwl:hasOBONamespace>GAZ</oboInOwl:hasOBONamespace>
        <oboInOwl:id>GAZ:00471835</oboInOwl:id>
        <rdfs:label>Wole Oko</rdfs:label>
    </owl:NamedIndividual>
    


    <!-- http://purl.obolibrary.org/obo/GAZ_00471838 -->

    <owl:NamedIndividual rdf:about="http://purl.obolibrary.org/obo/GAZ_00471838">
        <obo:RO_0001025 rdf:resource="http://purl.obolibrary.org/obo/GAZ_00061762"/>
        <obo:IAO_0000115>A protected area.</obo:IAO_0000115>
        <oboInOwl:hasOBONamespace>GAZ</oboInOwl:hasOBONamespace>
        <oboInOwl:id>GAZ:00471838</oboInOwl:id>
        <rdfs:label>Park Krajobrazowy Beskidu Malego</rdfs:label>
    </owl:NamedIndividual>
    


    <!-- http://purl.obolibrary.org/obo/GAZ_00477830 -->

    <owl:NamedIndividual rdf:about="http://purl.obolibrary.org/obo/GAZ_00477830">
        <obo:RO_0001025 rdf:resource="http://purl.obolibrary.org/obo/GAZ_00477999"/>
        <obo:IAO_0000115>A protected area.</obo:IAO_0000115>
        <oboInOwl:hasOBONamespace>GAZ</oboInOwl:hasOBONamespace>
        <oboInOwl:id>GAZ:00477830</oboInOwl:id>
        <rdfs:label>Rezerwat przyrody Kamien nad Jasliskami</rdfs:label>
    </owl:NamedIndividual>
    


    <!-- http://purl.obolibrary.org/obo/GAZ_00477831 -->

    <owl:NamedIndividual rdf:about="http://purl.obolibrary.org/obo/GAZ_00477831">
        <obo:RO_0001025 rdf:resource="http://purl.obolibrary.org/obo/GAZ_00061932"/>
        <obo:RO_0001025 rdf:resource="http://purl.obolibrary.org/obo/GAZ_00477999"/>
        <obo:IAO_0000115>A protected area.</obo:IAO_0000115>
        <oboInOwl:hasOBONamespace>GAZ</oboInOwl:hasOBONamespace>
        <oboInOwl:id>GAZ:00477831</oboInOwl:id>
        <rdfs:label>Rezerwat przyrody Modrzyna</rdfs:label>
    </owl:NamedIndividual>
    


    <!-- http://purl.obolibrary.org/obo/GAZ_00477832 -->

    <owl:NamedIndividual rdf:about="http://purl.obolibrary.org/obo/GAZ_00477832">
        <obo:RO_0001025 rdf:resource="http://purl.obolibrary.org/obo/GAZ_00477999"/>
        <obo:IAO_0000115>A protected area.</obo:IAO_0000115>
        <oboInOwl:hasOBONamespace>GAZ</oboInOwl:hasOBONamespace>
        <oboInOwl:id>GAZ:00477832</oboInOwl:id>
        <rdfs:label>Rezerwat przyrody Przelom Jasiolki</rdfs:label>
    </owl:NamedIndividual>
    


    <!-- http://purl.obolibrary.org/obo/GAZ_00477834 -->

    <owl:NamedIndividual rdf:about="http://purl.obolibrary.org/obo/GAZ_00477834">
        <obo:RO_0001025 rdf:resource="http://purl.obolibrary.org/obo/GAZ_00477999"/>
        <obo:IAO_0000115>A protected area.</obo:IAO_0000115>
        <oboInOwl:hasOBONamespace>GAZ</oboInOwl:hasOBONamespace>
        <oboInOwl:id>GAZ:00477834</oboInOwl:id>
        <rdfs:label>Rezerwat przyrody Wadernik</rdfs:label>
    </owl:NamedIndividual>
    


    <!-- http://purl.obolibrary.org/obo/GAZ_00477999 -->

    <owl:NamedIndividual rdf:about="http://purl.obolibrary.org/obo/GAZ_00477999">
        <obo:RO_0001025 rdf:resource="http://purl.obolibrary.org/obo/GAZ_00061932"/>
        <obo:IAO_0000115>A protected area.</obo:IAO_0000115>
        <oboInOwl:hasOBONamespace>GAZ</oboInOwl:hasOBONamespace>
        <oboInOwl:id>GAZ:00477999</oboInOwl:id>
        <rdfs:label>Jasliski Park Krajobrazowy</rdfs:label>
    </owl:NamedIndividual>
    


    <!-- http://purl.obolibrary.org/obo/GAZ_00478000 -->

    <owl:NamedIndividual rdf:about="http://purl.obolibrary.org/obo/GAZ_00478000">
        <obo:RO_0001025 rdf:resource="http://purl.obolibrary.org/obo/GAZ_00477999"/>
        <obo:IAO_0000115>A protected area.</obo:IAO_0000115>
        <oboInOwl:hasOBONamespace>GAZ</oboInOwl:hasOBONamespace>
        <oboInOwl:id>GAZ:00478000</oboInOwl:id>
        <rdfs:label>Rezerwat przyrody Zrodliska Jasiolki</rdfs:label>
    </owl:NamedIndividual>
    


    <!-- http://purl.obolibrary.org/obo/GAZ_00480341 -->

    <owl:NamedIndividual rdf:about="http://purl.obolibrary.org/obo/GAZ_00480341">
        <obo:IAO_0000115>A reservoir.</obo:IAO_0000115>
        <oboInOwl:hasOBONamespace>GAZ</oboInOwl:hasOBONamespace>
        <oboInOwl:id>GAZ:00480341</oboInOwl:id>
        <rdfs:label>Jezioro Czorsztynskie</rdfs:label>
    </owl:NamedIndividual>
    


    <!-- http://purl.obolibrary.org/obo/GAZ_00480508 -->

    <owl:NamedIndividual rdf:about="http://purl.obolibrary.org/obo/GAZ_00480508">
        <obo:IAO_0000115>A reservoir.</obo:IAO_0000115>
        <oboInOwl:hasOBONamespace>GAZ</oboInOwl:hasOBONamespace>
        <oboInOwl:id>GAZ:00480508</oboInOwl:id>
        <rdfs:label>Jezioro Roznowskie</rdfs:label>
    </owl:NamedIndividual>
    


    <!-- http://purl.obolibrary.org/obo/GAZ_00481026 -->

    <owl:NamedIndividual rdf:about="http://purl.obolibrary.org/obo/GAZ_00481026">
        <obo:RO_0001025 rdf:resource="http://purl.obolibrary.org/obo/GAZ_00481031"/>
        <obo:IAO_0000115>Lakes.</obo:IAO_0000115>
        <oboInOwl:hasOBONamespace>GAZ</oboInOwl:hasOBONamespace>
        <oboInOwl:id>GAZ:00481026</oboInOwl:id>
        <rdfs:label>Czerwone Stawki Gasienicowe</rdfs:label>
    </owl:NamedIndividual>
    


    <!-- http://purl.obolibrary.org/obo/GAZ_00481027 -->

    <owl:NamedIndividual rdf:about="http://purl.obolibrary.org/obo/GAZ_00481027">
        <obo:RO_0001025 rdf:resource="http://purl.obolibrary.org/obo/GAZ_00481026"/>
        <obo:IAO_0000115>A lake.</obo:IAO_0000115>
        <oboInOwl:hasOBONamespace>GAZ</oboInOwl:hasOBONamespace>
        <oboInOwl:id>GAZ:00481027</oboInOwl:id>
        <rdfs:label>Wyzni Czerwony Stawek</rdfs:label>
    </owl:NamedIndividual>
    


    <!-- http://purl.obolibrary.org/obo/GAZ_00481028 -->

    <owl:NamedIndividual rdf:about="http://purl.obolibrary.org/obo/GAZ_00481028">
        <obo:RO_0001025 rdf:resource="http://purl.obolibrary.org/obo/GAZ_00481026"/>
        <obo:IAO_0000115>A lake.</obo:IAO_0000115>
        <oboInOwl:hasOBONamespace>GAZ</oboInOwl:hasOBONamespace>
        <oboInOwl:id>GAZ:00481028</oboInOwl:id>
        <rdfs:label>Nizni Czerwony Stawek</rdfs:label>
    </owl:NamedIndividual>
    


    <!-- http://purl.obolibrary.org/obo/GAZ_00481029 -->

    <owl:NamedIndividual rdf:about="http://purl.obolibrary.org/obo/GAZ_00481029">
        <obo:IAO_0000115>A lake.</obo:IAO_0000115>
        <oboInOwl:hasOBONamespace>GAZ</oboInOwl:hasOBONamespace>
        <oboInOwl:id>GAZ:00481029</oboInOwl:id>
        <rdfs:label>Czerwony Staw Panszczycki</rdfs:label>
    </owl:NamedIndividual>
    


    <!-- http://purl.obolibrary.org/obo/GAZ_00481030 -->

    <owl:NamedIndividual rdf:about="http://purl.obolibrary.org/obo/GAZ_00481030">
        <obo:RO_0001025 rdf:resource="http://purl.obolibrary.org/obo/GAZ_00056820"/>
        <obo:IAO_0000115>Five lakes.</obo:IAO_0000115>
        <oboInOwl:hasOBONamespace>GAZ</oboInOwl:hasOBONamespace>
        <oboInOwl:id>GAZ:00481030</oboInOwl:id>
        <rdfs:label>Dudowe Stawki</rdfs:label>
    </owl:NamedIndividual>
    


    <!-- http://purl.obolibrary.org/obo/GAZ_00481031 -->

    <owl:NamedIndividual rdf:about="http://purl.obolibrary.org/obo/GAZ_00481031">
        <obo:IAO_0000115>Lakes in Dolina Gasienicowa.</obo:IAO_0000115>
        <oboInOwl:hasOBONamespace>GAZ</oboInOwl:hasOBONamespace>
        <oboInOwl:id>GAZ:00481031</oboInOwl:id>
        <rdfs:label>Gasienicowe Stawy</rdfs:label>
    </owl:NamedIndividual>
    


    <!-- http://purl.obolibrary.org/obo/GAZ_00481032 -->

    <owl:NamedIndividual rdf:about="http://purl.obolibrary.org/obo/GAZ_00481032">
        <obo:RO_0001025 rdf:resource="http://purl.obolibrary.org/obo/GAZ_00481031"/>
        <obo:IAO_0000115>Two lakes.</obo:IAO_0000115>
        <oboInOwl:hasOBONamespace>GAZ</oboInOwl:hasOBONamespace>
        <oboInOwl:id>GAZ:00481032</oboInOwl:id>
        <rdfs:label>Dwoisty Staw Gasienicowy</rdfs:label>
    </owl:NamedIndividual>
    


    <!-- http://purl.obolibrary.org/obo/GAZ_00481033 -->

    <owl:NamedIndividual rdf:about="http://purl.obolibrary.org/obo/GAZ_00481033">
        <obo:RO_0001025 rdf:resource="http://purl.obolibrary.org/obo/GAZ_00481032"/>
        <obo:IAO_0000115>A lake.</obo:IAO_0000115>
        <oboInOwl:hasOBONamespace>GAZ</oboInOwl:hasOBONamespace>
        <oboInOwl:id>GAZ:00481033</oboInOwl:id>
        <rdfs:label>Dwoisty Staw Wschodni</rdfs:label>
    </owl:NamedIndividual>
    


    <!-- http://purl.obolibrary.org/obo/GAZ_00481034 -->

    <owl:NamedIndividual rdf:about="http://purl.obolibrary.org/obo/GAZ_00481034">
        <obo:RO_0001025 rdf:resource="http://purl.obolibrary.org/obo/GAZ_00481032"/>
        <obo:IAO_0000115>A lake.</obo:IAO_0000115>
        <oboInOwl:hasOBONamespace>GAZ</oboInOwl:hasOBONamespace>
        <oboInOwl:id>GAZ:00481034</oboInOwl:id>
        <rdfs:label>Dwoisty Staw Zachodni</rdfs:label>
    </owl:NamedIndividual>
    


    <!-- http://purl.obolibrary.org/obo/GAZ_00481035 -->

    <owl:NamedIndividual rdf:about="http://purl.obolibrary.org/obo/GAZ_00481035">
        <obo:RO_0001025 rdf:resource="http://purl.obolibrary.org/obo/GAZ_00481031"/>
        <obo:IAO_0000115>A lake.</obo:IAO_0000115>
        <oboInOwl:hasOBONamespace>GAZ</oboInOwl:hasOBONamespace>
        <oboInOwl:id>GAZ:00481035</oboInOwl:id>
        <rdfs:label>Zielony Staw Gasienicowy</rdfs:label>
    </owl:NamedIndividual>
    


    <!-- http://purl.obolibrary.org/obo/GAZ_00481036 -->

    <owl:NamedIndividual rdf:about="http://purl.obolibrary.org/obo/GAZ_00481036">
        <obo:RO_0001025 rdf:resource="http://purl.obolibrary.org/obo/GAZ_00056820"/>
        <obo:IAO_0000115>A valley.</obo:IAO_0000115>
        <oboInOwl:hasOBONamespace>GAZ</oboInOwl:hasOBONamespace>
        <oboInOwl:id>GAZ:00481036</oboInOwl:id>
        <rdfs:label>Dolina Goryczkowa</rdfs:label>
    </owl:NamedIndividual>
    


    <!-- http://purl.obolibrary.org/obo/GAZ_00481037 -->

    <owl:NamedIndividual rdf:about="http://purl.obolibrary.org/obo/GAZ_00481037">
        <obo:RO_0001025 rdf:resource="http://purl.obolibrary.org/obo/GAZ_00481031"/>
        <obo:IAO_0000115>A lake.</obo:IAO_0000115>
        <oboInOwl:hasOBONamespace>GAZ</oboInOwl:hasOBONamespace>
        <oboInOwl:id>GAZ:00481037</oboInOwl:id>
        <rdfs:label>Kurtkowiec</rdfs:label>
    </owl:NamedIndividual>
    


    <!-- http://purl.obolibrary.org/obo/GAZ_00481038 -->

    <owl:NamedIndividual rdf:about="http://purl.obolibrary.org/obo/GAZ_00481038">
        <obo:RO_0001025 rdf:resource="http://purl.obolibrary.org/obo/GAZ_00481031"/>
        <obo:IAO_0000115>A lake.</obo:IAO_0000115>
        <oboInOwl:hasOBONamespace>GAZ</oboInOwl:hasOBONamespace>
        <oboInOwl:id>GAZ:00481038</oboInOwl:id>
        <rdfs:label>Zadni Staw Gasienicowy</rdfs:label>
    </owl:NamedIndividual>
    


    <!-- http://purl.obolibrary.org/obo/GAZ_00481039 -->

    <owl:NamedIndividual rdf:about="http://purl.obolibrary.org/obo/GAZ_00481039">
        <obo:RO_0001025 rdf:resource="http://purl.obolibrary.org/obo/GAZ_00481031"/>
        <obo:IAO_0000115>A lake.</obo:IAO_0000115>
        <oboInOwl:hasOBONamespace>GAZ</oboInOwl:hasOBONamespace>
        <oboInOwl:id>GAZ:00481039</oboInOwl:id>
        <rdfs:label>Litworowy Staw Gasienicowy</rdfs:label>
    </owl:NamedIndividual>
    


    <!-- http://purl.obolibrary.org/obo/GAZ_00481040 -->

    <owl:NamedIndividual rdf:about="http://purl.obolibrary.org/obo/GAZ_00481040">
        <obo:RO_0001025 rdf:resource="http://purl.obolibrary.org/obo/GAZ_00481031"/>
        <obo:IAO_0000115>A lake.</obo:IAO_0000115>
        <oboInOwl:hasOBONamespace>GAZ</oboInOwl:hasOBONamespace>
        <oboInOwl:id>GAZ:00481040</oboInOwl:id>
        <rdfs:label>Mokra Jama</rdfs:label>
    </owl:NamedIndividual>
    


    <!-- http://purl.obolibrary.org/obo/GAZ_00481041 -->

    <owl:NamedIndividual rdf:about="http://purl.obolibrary.org/obo/GAZ_00481041">
        <obo:RO_0001025 rdf:resource="http://purl.obolibrary.org/obo/GAZ_00481031"/>
        <obo:IAO_0000115>A lake.</obo:IAO_0000115>
        <oboInOwl:hasOBONamespace>GAZ</oboInOwl:hasOBONamespace>
        <oboInOwl:id>GAZ:00481041</oboInOwl:id>
        <rdfs:label>Kotlinowy Stawek</rdfs:label>
    </owl:NamedIndividual>
    


    <!-- http://purl.obolibrary.org/obo/GAZ_00481042 -->

    <owl:NamedIndividual rdf:about="http://purl.obolibrary.org/obo/GAZ_00481042">
        <obo:RO_0001025 rdf:resource="http://purl.obolibrary.org/obo/GAZ_00481031"/>
        <obo:IAO_0000115>Four lakes.</obo:IAO_0000115>
        <oboInOwl:hasOBONamespace>GAZ</oboInOwl:hasOBONamespace>
        <oboInOwl:id>GAZ:00481042</oboInOwl:id>
        <rdfs:label>Dwoisniaczek</rdfs:label>
    </owl:NamedIndividual>
    


    <!-- http://purl.obolibrary.org/obo/GAZ_00481043 -->

    <owl:NamedIndividual rdf:about="http://purl.obolibrary.org/obo/GAZ_00481043">
        <obo:RO_0001025 rdf:resource="http://purl.obolibrary.org/obo/GAZ_00481031"/>
        <obo:IAO_0000115>Three lakes.</obo:IAO_0000115>
        <oboInOwl:hasOBONamespace>GAZ</oboInOwl:hasOBONamespace>
        <oboInOwl:id>GAZ:00481043</oboInOwl:id>
        <rdfs:label>Troisniak</rdfs:label>
    </owl:NamedIndividual>
    


    <!-- http://purl.obolibrary.org/obo/GAZ_00481044 -->

    <owl:NamedIndividual rdf:about="http://purl.obolibrary.org/obo/GAZ_00481044">
        <obo:RO_0001025 rdf:resource="http://purl.obolibrary.org/obo/GAZ_00481031"/>
        <obo:IAO_0000115>A lake.</obo:IAO_0000115>
        <oboInOwl:hasOBONamespace>GAZ</oboInOwl:hasOBONamespace>
        <oboInOwl:id>GAZ:00481044</oboInOwl:id>
        <rdfs:label>Dwoisniak</rdfs:label>
    </owl:NamedIndividual>
    


    <!-- http://purl.obolibrary.org/obo/GAZ_00481045 -->

    <owl:NamedIndividual rdf:about="http://purl.obolibrary.org/obo/GAZ_00481045">
        <obo:RO_0001025 rdf:resource="http://purl.obolibrary.org/obo/GAZ_00481031"/>
        <obo:IAO_0000115>A lake.</obo:IAO_0000115>
        <oboInOwl:hasOBONamespace>GAZ</oboInOwl:hasOBONamespace>
        <oboInOwl:id>GAZ:00481045</oboInOwl:id>
        <rdfs:label>Jedyniak</rdfs:label>
    </owl:NamedIndividual>
    


    <!-- http://purl.obolibrary.org/obo/GAZ_00481046 -->

    <owl:NamedIndividual rdf:about="http://purl.obolibrary.org/obo/GAZ_00481046">
        <obo:RO_0001025 rdf:resource="http://purl.obolibrary.org/obo/GAZ_00481031"/>
        <obo:IAO_0000115>A lake.</obo:IAO_0000115>
        <oboInOwl:hasOBONamespace>GAZ</oboInOwl:hasOBONamespace>
        <oboInOwl:id>GAZ:00481046</oboInOwl:id>
        <rdfs:label>Samotniak</rdfs:label>
    </owl:NamedIndividual>
    


    <!-- http://purl.obolibrary.org/obo/GAZ_00481047 -->

    <owl:NamedIndividual rdf:about="http://purl.obolibrary.org/obo/GAZ_00481047">
        <obo:RO_0001025 rdf:resource="http://purl.obolibrary.org/obo/GAZ_00481043"/>
        <obo:IAO_0000115>A lake.</obo:IAO_0000115>
        <oboInOwl:hasOBONamespace>GAZ</oboInOwl:hasOBONamespace>
        <oboInOwl:id>GAZ:00481047</oboInOwl:id>
        <rdfs:label>Troisniak Nizni</rdfs:label>
    </owl:NamedIndividual>
    


    <!-- http://purl.obolibrary.org/obo/GAZ_00481048 -->

    <owl:NamedIndividual rdf:about="http://purl.obolibrary.org/obo/GAZ_00481048">
        <obo:RO_0001025 rdf:resource="http://purl.obolibrary.org/obo/GAZ_00481043"/>
        <obo:IAO_0000115>A lake.</obo:IAO_0000115>
        <oboInOwl:hasOBONamespace>GAZ</oboInOwl:hasOBONamespace>
        <oboInOwl:id>GAZ:00481048</oboInOwl:id>
        <rdfs:label>Troisniak Posredni</rdfs:label>
    </owl:NamedIndividual>
    


    <!-- http://purl.obolibrary.org/obo/GAZ_00481049 -->

    <owl:NamedIndividual rdf:about="http://purl.obolibrary.org/obo/GAZ_00481049">
        <obo:RO_0001025 rdf:resource="http://purl.obolibrary.org/obo/GAZ_00481043"/>
        <obo:IAO_0000115>A lake.</obo:IAO_0000115>
        <oboInOwl:hasOBONamespace>GAZ</oboInOwl:hasOBONamespace>
        <oboInOwl:id>GAZ:00481049</oboInOwl:id>
        <rdfs:label>Troisniak Wyzni</rdfs:label>
    </owl:NamedIndividual>
    


    <!-- http://purl.obolibrary.org/obo/GAZ_00481050 -->

    <owl:NamedIndividual rdf:about="http://purl.obolibrary.org/obo/GAZ_00481050">
        <obo:RO_0001025 rdf:resource="http://purl.obolibrary.org/obo/GAZ_00481031"/>
        <obo:IAO_0000115>A lake.</obo:IAO_0000115>
        <oboInOwl:hasOBONamespace>GAZ</oboInOwl:hasOBONamespace>
        <oboInOwl:id>GAZ:00481050</oboInOwl:id>
        <rdfs:label>Zmarzly Staw Gasienicowy</rdfs:label>
    </owl:NamedIndividual>
    


    <!-- http://purl.obolibrary.org/obo/GAZ_00481051 -->

    <owl:NamedIndividual rdf:about="http://purl.obolibrary.org/obo/GAZ_00481051">
        <obo:IAO_0000115>Two lakes.</obo:IAO_0000115>
        <oboInOwl:hasOBONamespace>GAZ</oboInOwl:hasOBONamespace>
        <oboInOwl:id>GAZ:00481051</oboInOwl:id>
        <rdfs:label>Dwoisniak</rdfs:label>
    </owl:NamedIndividual>
    


    <!-- http://purl.obolibrary.org/obo/GAZ_00481052 -->

    <owl:NamedIndividual rdf:about="http://purl.obolibrary.org/obo/GAZ_00481052">
        <obo:RO_0001025 rdf:resource="http://purl.obolibrary.org/obo/GAZ_00481051"/>
        <obo:IAO_0000115>A lake.</obo:IAO_0000115>
        <oboInOwl:hasOBONamespace>GAZ</oboInOwl:hasOBONamespace>
        <oboInOwl:id>GAZ:00481052</oboInOwl:id>
        <rdfs:label>Dwoisniak Nizni</rdfs:label>
    </owl:NamedIndividual>
    


    <!-- http://purl.obolibrary.org/obo/GAZ_00481053 -->

    <owl:NamedIndividual rdf:about="http://purl.obolibrary.org/obo/GAZ_00481053">
        <obo:RO_0001025 rdf:resource="http://purl.obolibrary.org/obo/GAZ_00481051"/>
        <obo:IAO_0000115>A lake.</obo:IAO_0000115>
        <oboInOwl:hasOBONamespace>GAZ</oboInOwl:hasOBONamespace>
        <oboInOwl:id>GAZ:00481053</oboInOwl:id>
        <rdfs:label>Dwoisniak Wyzni</rdfs:label>
    </owl:NamedIndividual>
    


    <!-- http://purl.obolibrary.org/obo/GAZ_00481054 -->

    <owl:NamedIndividual rdf:about="http://purl.obolibrary.org/obo/GAZ_00481054">
        <obo:RO_0001025 rdf:resource="http://purl.obolibrary.org/obo/GAZ_00481031"/>
        <obo:IAO_0000115>A lake.</obo:IAO_0000115>
        <oboInOwl:hasOBONamespace>GAZ</oboInOwl:hasOBONamespace>
        <oboInOwl:id>GAZ:00481054</oboInOwl:id>
        <rdfs:label>Dlugi Staw Gasienicowy</rdfs:label>
    </owl:NamedIndividual>
    


    <!-- http://purl.obolibrary.org/obo/GAZ_00481058 -->

    <owl:NamedIndividual rdf:about="http://purl.obolibrary.org/obo/GAZ_00481058">
        <obo:IAO_0000115>A lake.</obo:IAO_0000115>
        <oboInOwl:hasOBONamespace>GAZ</oboInOwl:hasOBONamespace>
        <oboInOwl:id>GAZ:00481058</oboInOwl:id>
        <rdfs:label>Kosowinowe Oczko</rdfs:label>
    </owl:NamedIndividual>
    


    <!-- http://purl.obolibrary.org/obo/GAZ_00481059 -->

    <owl:NamedIndividual rdf:about="http://purl.obolibrary.org/obo/GAZ_00481059">
        <obo:RO_0001025 rdf:resource="http://purl.obolibrary.org/obo/GAZ_00061848"/>
        <obo:IAO_0000115>A valley.</obo:IAO_0000115>
        <oboInOwl:hasOBONamespace>GAZ</oboInOwl:hasOBONamespace>
        <oboInOwl:id>GAZ:00481059</oboInOwl:id>
        <rdfs:label>Dolina Lejowa</rdfs:label>
    </owl:NamedIndividual>
    


    <!-- http://purl.obolibrary.org/obo/GAZ_00481060 -->

    <owl:NamedIndividual rdf:about="http://purl.obolibrary.org/obo/GAZ_00481060">
        <obo:RO_0001025 rdf:resource="http://purl.obolibrary.org/obo/GAZ_00056820"/>
        <obo:IAO_0000115>A valley.</obo:IAO_0000115>
        <oboInOwl:hasOBONamespace>GAZ</oboInOwl:hasOBONamespace>
        <oboInOwl:id>GAZ:00481060</oboInOwl:id>
        <rdfs:label>Dolina Chocholowska</rdfs:label>
    </owl:NamedIndividual>
    


    <!-- http://purl.obolibrary.org/obo/GAZ_00481061 -->

    <owl:NamedIndividual rdf:about="http://purl.obolibrary.org/obo/GAZ_00481061">
        <obo:RO_0001025 rdf:resource="http://purl.obolibrary.org/obo/GAZ_00056820"/>
        <obo:IAO_0000115>A valley.</obo:IAO_0000115>
        <oboInOwl:hasOBONamespace>GAZ</oboInOwl:hasOBONamespace>
        <oboInOwl:id>GAZ:00481061</oboInOwl:id>
        <rdfs:label>Dolina Koscieliska</rdfs:label>
    </owl:NamedIndividual>
    


    <!-- http://purl.obolibrary.org/obo/GAZ_00481062 -->

    <owl:NamedIndividual rdf:about="http://purl.obolibrary.org/obo/GAZ_00481062">
        <obo:RO_0001025 rdf:resource="http://purl.obolibrary.org/obo/GAZ_00481059"/>
        <obo:IAO_0000115>A lake.</obo:IAO_0000115>
        <oboInOwl:hasOBONamespace>GAZ</oboInOwl:hasOBONamespace>
        <oboInOwl:id>GAZ:00481062</oboInOwl:id>
        <rdfs:label>Maturowy Stawek</rdfs:label>
    </owl:NamedIndividual>
    


    <!-- http://purl.obolibrary.org/obo/GAZ_00481063 -->

    <owl:NamedIndividual rdf:about="http://purl.obolibrary.org/obo/GAZ_00481063">
        <obo:RO_0001025 rdf:resource="http://purl.obolibrary.org/obo/GAZ_00061848"/>
        <obo:IAO_0000115>A valley.</obo:IAO_0000115>
        <oboInOwl:hasOBONamespace>GAZ</oboInOwl:hasOBONamespace>
        <oboInOwl:id>GAZ:00481063</oboInOwl:id>
        <rdfs:label>Dolina Pieciu Stawow Polskich</rdfs:label>
    </owl:NamedIndividual>
    


    <!-- http://purl.obolibrary.org/obo/GAZ_00481064 -->

    <owl:NamedIndividual rdf:about="http://purl.obolibrary.org/obo/GAZ_00481064">
        <obo:RO_0001025 rdf:resource="http://purl.obolibrary.org/obo/GAZ_00481063"/>
        <obo:IAO_0000115>A lake.</obo:IAO_0000115>
        <oboInOwl:hasOBONamespace>GAZ</oboInOwl:hasOBONamespace>
        <oboInOwl:id>GAZ:00481064</oboInOwl:id>
        <rdfs:label>Czarny Staw Polski</rdfs:label>
    </owl:NamedIndividual>
    


    <!-- http://purl.obolibrary.org/obo/GAZ_00481065 -->

    <owl:NamedIndividual rdf:about="http://purl.obolibrary.org/obo/GAZ_00481065">
        <obo:RO_0001025 rdf:resource="http://purl.obolibrary.org/obo/GAZ_00481063"/>
        <obo:IAO_0000115>Three lakes.</obo:IAO_0000115>
        <oboInOwl:hasOBONamespace>GAZ</oboInOwl:hasOBONamespace>
        <oboInOwl:id>GAZ:00481065</oboInOwl:id>
        <rdfs:label>Szpiglasowe Stawki</rdfs:label>
    </owl:NamedIndividual>
    


    <!-- http://purl.obolibrary.org/obo/GAZ_00481066 -->

    <owl:NamedIndividual rdf:about="http://purl.obolibrary.org/obo/GAZ_00481066">
        <obo:IAO_0000115>Two lakes.</obo:IAO_0000115>
        <oboInOwl:hasOBONamespace>GAZ</oboInOwl:hasOBONamespace>
        <oboInOwl:id>GAZ:00481066</oboInOwl:id>
        <rdfs:label>Siwe Stawki</rdfs:label>
    </owl:NamedIndividual>
    


    <!-- http://purl.obolibrary.org/obo/GAZ_00481067 -->

    <owl:NamedIndividual rdf:about="http://purl.obolibrary.org/obo/GAZ_00481067">
        <obo:IAO_0000115>A lake.</obo:IAO_0000115>
        <oboInOwl:hasOBONamespace>GAZ</oboInOwl:hasOBONamespace>
        <oboInOwl:id>GAZ:00481067</oboInOwl:id>
        <rdfs:label>Smreczynski Staw</rdfs:label>
    </owl:NamedIndividual>
    


    <!-- http://purl.obolibrary.org/obo/GAZ_00481069 -->

    <owl:NamedIndividual rdf:about="http://purl.obolibrary.org/obo/GAZ_00481069">
        <obo:RO_0001025 rdf:resource="http://purl.obolibrary.org/obo/GAZ_00481087"/>
        <obo:IAO_0000115>A lake.</obo:IAO_0000115>
        <oboInOwl:hasOBONamespace>GAZ</oboInOwl:hasOBONamespace>
        <oboInOwl:id>GAZ:00481069</oboInOwl:id>
        <rdfs:label>Anusine Oczko</rdfs:label>
    </owl:NamedIndividual>
    


    <!-- http://purl.obolibrary.org/obo/GAZ_00481070 -->

    <owl:NamedIndividual rdf:about="http://purl.obolibrary.org/obo/GAZ_00481070">
        <obo:RO_0001025 rdf:resource="http://purl.obolibrary.org/obo/GAZ_00481086"/>
        <obo:IAO_0000115>Lakes.</obo:IAO_0000115>
        <oboInOwl:hasOBONamespace>GAZ</oboInOwl:hasOBONamespace>
        <oboInOwl:id>GAZ:00481070</oboInOwl:id>
        <rdfs:label>Wyznie Mnichowe Stawki</rdfs:label>
    </owl:NamedIndividual>
    


    <!-- http://purl.obolibrary.org/obo/GAZ_00481071 -->

    <owl:NamedIndividual rdf:about="http://purl.obolibrary.org/obo/GAZ_00481071">
        <obo:RO_0001025 rdf:resource="http://purl.obolibrary.org/obo/GAZ_00481070"/>
        <obo:IAO_0000115>A lake.</obo:IAO_0000115>
        <oboInOwl:hasOBONamespace>GAZ</oboInOwl:hasOBONamespace>
        <oboInOwl:id>GAZ:00481071</oboInOwl:id>
        <rdfs:label>Wyzni Mnichowy Stawek I</rdfs:label>
    </owl:NamedIndividual>
    


    <!-- http://purl.obolibrary.org/obo/GAZ_00481072 -->

    <owl:NamedIndividual rdf:about="http://purl.obolibrary.org/obo/GAZ_00481072">
        <obo:RO_0001025 rdf:resource="http://purl.obolibrary.org/obo/GAZ_00481070"/>
        <obo:IAO_0000115>A lake.</obo:IAO_0000115>
        <oboInOwl:hasOBONamespace>GAZ</oboInOwl:hasOBONamespace>
        <oboInOwl:id>GAZ:00481072</oboInOwl:id>
        <rdfs:label>Wyzni Mnichowy Stawek II</rdfs:label>
    </owl:NamedIndividual>
    


    <!-- http://purl.obolibrary.org/obo/GAZ_00481073 -->

    <owl:NamedIndividual rdf:about="http://purl.obolibrary.org/obo/GAZ_00481073">
        <obo:RO_0001025 rdf:resource="http://purl.obolibrary.org/obo/GAZ_00481070"/>
        <obo:IAO_0000115>A lake.</obo:IAO_0000115>
        <oboInOwl:hasOBONamespace>GAZ</oboInOwl:hasOBONamespace>
        <oboInOwl:id>GAZ:00481073</oboInOwl:id>
        <rdfs:label>Wyzni Mnichowy Stawek III</rdfs:label>
    </owl:NamedIndividual>
    


    <!-- http://purl.obolibrary.org/obo/GAZ_00481074 -->

    <owl:NamedIndividual rdf:about="http://purl.obolibrary.org/obo/GAZ_00481074">
        <obo:RO_0001025 rdf:resource="http://purl.obolibrary.org/obo/GAZ_00481070"/>
        <obo:IAO_0000115>A lake.</obo:IAO_0000115>
        <oboInOwl:hasOBONamespace>GAZ</oboInOwl:hasOBONamespace>
        <oboInOwl:id>GAZ:00481074</oboInOwl:id>
        <rdfs:label>Wyzni Mnichowy Stawek IV</rdfs:label>
    </owl:NamedIndividual>
    


    <!-- http://purl.obolibrary.org/obo/GAZ_00481075 -->

    <owl:NamedIndividual rdf:about="http://purl.obolibrary.org/obo/GAZ_00481075">
        <obo:RO_0001025 rdf:resource="http://purl.obolibrary.org/obo/GAZ_00481070"/>
        <obo:IAO_0000115>A lake.</obo:IAO_0000115>
        <oboInOwl:hasOBONamespace>GAZ</oboInOwl:hasOBONamespace>
        <oboInOwl:id>GAZ:00481075</oboInOwl:id>
        <rdfs:label>Wyzni Mnichowy Stawek V</rdfs:label>
    </owl:NamedIndividual>
    


    <!-- http://purl.obolibrary.org/obo/GAZ_00481076 -->

    <owl:NamedIndividual rdf:about="http://purl.obolibrary.org/obo/GAZ_00481076">
        <obo:RO_0001025 rdf:resource="http://purl.obolibrary.org/obo/GAZ_00481070"/>
        <obo:IAO_0000115>A lake.</obo:IAO_0000115>
        <oboInOwl:hasOBONamespace>GAZ</oboInOwl:hasOBONamespace>
        <oboInOwl:id>GAZ:00481076</oboInOwl:id>
        <rdfs:label>Wyzni Mnichowy Stawek VI</rdfs:label>
    </owl:NamedIndividual>
    


    <!-- http://purl.obolibrary.org/obo/GAZ_00481077 -->

    <owl:NamedIndividual rdf:about="http://purl.obolibrary.org/obo/GAZ_00481077">
        <obo:RO_0001025 rdf:resource="http://purl.obolibrary.org/obo/GAZ_00481070"/>
        <obo:IAO_0000115>A lake.</obo:IAO_0000115>
        <oboInOwl:hasOBONamespace>GAZ</oboInOwl:hasOBONamespace>
        <oboInOwl:id>GAZ:00481077</oboInOwl:id>
        <rdfs:label>Wyzni Mnichowy Stawek VII</rdfs:label>
    </owl:NamedIndividual>
    


    <!-- http://purl.obolibrary.org/obo/GAZ_00481078 -->

    <owl:NamedIndividual rdf:about="http://purl.obolibrary.org/obo/GAZ_00481078">
        <obo:RO_0001025 rdf:resource="http://purl.obolibrary.org/obo/GAZ_00481070"/>
        <obo:IAO_0000115>A lake.</obo:IAO_0000115>
        <oboInOwl:hasOBONamespace>GAZ</oboInOwl:hasOBONamespace>
        <oboInOwl:id>GAZ:00481078</oboInOwl:id>
        <rdfs:label>Wyzni Mnichowy Stawek VIII</rdfs:label>
    </owl:NamedIndividual>
    


    <!-- http://purl.obolibrary.org/obo/GAZ_00481079 -->

    <owl:NamedIndividual rdf:about="http://purl.obolibrary.org/obo/GAZ_00481079">
        <obo:RO_0001025 rdf:resource="http://purl.obolibrary.org/obo/GAZ_00481070"/>
        <obo:IAO_0000115>A lake.</obo:IAO_0000115>
        <oboInOwl:hasOBONamespace>GAZ</oboInOwl:hasOBONamespace>
        <oboInOwl:id>GAZ:00481079</oboInOwl:id>
        <rdfs:label>Wyzni Mnichowy Stawek IX</rdfs:label>
    </owl:NamedIndividual>
    


    <!-- http://purl.obolibrary.org/obo/GAZ_00481081 -->

    <owl:NamedIndividual rdf:about="http://purl.obolibrary.org/obo/GAZ_00481081">
        <obo:IAO_0000115>A lake.</obo:IAO_0000115>
        <oboInOwl:hasOBONamespace>GAZ</oboInOwl:hasOBONamespace>
        <oboInOwl:id>GAZ:00481081</oboInOwl:id>
        <rdfs:label>Zabie Oko</rdfs:label>
    </owl:NamedIndividual>
    


    <!-- http://purl.obolibrary.org/obo/GAZ_00481082 -->

    <owl:NamedIndividual rdf:about="http://purl.obolibrary.org/obo/GAZ_00481082">
        <obo:IAO_0000115>A lake.</obo:IAO_0000115>
        <oboInOwl:hasOBONamespace>GAZ</oboInOwl:hasOBONamespace>
        <oboInOwl:id>GAZ:00481082</oboInOwl:id>
        <rdfs:label>Male Zabie Oko</rdfs:label>
    </owl:NamedIndividual>
    


    <!-- http://purl.obolibrary.org/obo/GAZ_00481083 -->

    <owl:NamedIndividual rdf:about="http://purl.obolibrary.org/obo/GAZ_00481083">
        <obo:IAO_0000115>A lake.</obo:IAO_0000115>
        <oboInOwl:hasOBONamespace>GAZ</oboInOwl:hasOBONamespace>
        <oboInOwl:id>GAZ:00481083</oboInOwl:id>
        <rdfs:label>Male Morskie Oko</rdfs:label>
    </owl:NamedIndividual>
    


    <!-- http://purl.obolibrary.org/obo/GAZ_00481084 -->

    <owl:NamedIndividual rdf:about="http://purl.obolibrary.org/obo/GAZ_00481084">
        <obo:IAO_0000115>A lake.</obo:IAO_0000115>
        <oboInOwl:hasOBONamespace>GAZ</oboInOwl:hasOBONamespace>
        <oboInOwl:id>GAZ:00481084</oboInOwl:id>
        <rdfs:label>Rybie Stawki</rdfs:label>
    </owl:NamedIndividual>
    


    <!-- http://purl.obolibrary.org/obo/GAZ_00481086 -->

    <owl:NamedIndividual rdf:about="http://purl.obolibrary.org/obo/GAZ_00481086">
        <obo:IAO_0000115>A lake.</obo:IAO_0000115>
        <oboInOwl:hasOBONamespace>GAZ</oboInOwl:hasOBONamespace>
        <oboInOwl:id>GAZ:00481086</oboInOwl:id>
        <rdfs:label>Zadni Mnichowy Stawek</rdfs:label>
    </owl:NamedIndividual>
    


    <!-- http://purl.obolibrary.org/obo/GAZ_00481087 -->

    <owl:NamedIndividual rdf:about="http://purl.obolibrary.org/obo/GAZ_00481087">
        <obo:RO_0001025 rdf:resource="http://purl.obolibrary.org/obo/GAZ_00056820"/>
        <obo:IAO_0000115>A valley.</obo:IAO_0000115>
        <oboInOwl:hasOBONamespace>GAZ</oboInOwl:hasOBONamespace>
        <oboInOwl:id>GAZ:00481087</oboInOwl:id>
        <rdfs:label>Dolina Bystra</rdfs:label>
    </owl:NamedIndividual>
    


    <!-- http://purl.obolibrary.org/obo/GAZ_00481088 -->

    <owl:NamedIndividual rdf:about="http://purl.obolibrary.org/obo/GAZ_00481088">
        <obo:RO_0001025 rdf:resource="http://purl.obolibrary.org/obo/GAZ_00481087"/>
        <oboInOwl:hasOBONamespace>GAZ</oboInOwl:hasOBONamespace>
        <oboInOwl:id>GAZ:00481088</oboInOwl:id>
        <rdfs:label>Wielki Staw Bystry</rdfs:label>
    </owl:NamedIndividual>
    


    <!-- http://purl.obolibrary.org/obo/GAZ_00481089 -->

    <owl:NamedIndividual rdf:about="http://purl.obolibrary.org/obo/GAZ_00481089">
        <obo:RO_0001025 rdf:resource="http://purl.obolibrary.org/obo/GAZ_00481087"/>
        <oboInOwl:hasOBONamespace>GAZ</oboInOwl:hasOBONamespace>
        <oboInOwl:id>GAZ:00481089</oboInOwl:id>
        <rdfs:label>Dlugi Staw Bystry</rdfs:label>
    </owl:NamedIndividual>
    


    <!-- http://purl.obolibrary.org/obo/GAZ_00481090 -->

    <owl:NamedIndividual rdf:about="http://purl.obolibrary.org/obo/GAZ_00481090">
        <obo:RO_0001025 rdf:resource="http://purl.obolibrary.org/obo/GAZ_00481087"/>
        <oboInOwl:hasOBONamespace>GAZ</oboInOwl:hasOBONamespace>
        <oboInOwl:id>GAZ:00481090</oboInOwl:id>
        <rdfs:label>Maly Staw Bystry</rdfs:label>
    </owl:NamedIndividual>
    


    <!-- http://purl.obolibrary.org/obo/GAZ_00481091 -->

    <owl:NamedIndividual rdf:about="http://purl.obolibrary.org/obo/GAZ_00481091">
        <obo:RO_0001025 rdf:resource="http://purl.obolibrary.org/obo/GAZ_00481087"/>
        <oboInOwl:hasOBONamespace>GAZ</oboInOwl:hasOBONamespace>
        <oboInOwl:id>GAZ:00481091</oboInOwl:id>
        <rdfs:label>Nizni Staw Bystry</rdfs:label>
    </owl:NamedIndividual>
    


    <!-- http://purl.obolibrary.org/obo/GAZ_00481093 -->

    <owl:NamedIndividual rdf:about="http://purl.obolibrary.org/obo/GAZ_00481093">
        <obo:IAO_0000115>A lake.</obo:IAO_0000115>
        <oboInOwl:hasOBONamespace>GAZ</oboInOwl:hasOBONamespace>
        <oboInOwl:id>GAZ:00481093</oboInOwl:id>
        <rdfs:label>Baranie pliesko</rdfs:label>
    </owl:NamedIndividual>
    


    <!-- http://purl.obolibrary.org/obo/GAZ_00481094 -->

    <owl:NamedIndividual rdf:about="http://purl.obolibrary.org/obo/GAZ_00481094">
        <obo:RO_0001025 rdf:resource="http://purl.obolibrary.org/obo/GAZ_00007974"/>
        <obo:IAO_0000115>A valley.</obo:IAO_0000115>
        <oboInOwl:hasOBONamespace>GAZ</oboInOwl:hasOBONamespace>
        <oboInOwl:id>GAZ:00481094</oboInOwl:id>
        <rdfs:label>Batizovska dolina</rdfs:label>
    </owl:NamedIndividual>
    


    <!-- http://purl.obolibrary.org/obo/GAZ_00481095 -->

    <owl:NamedIndividual rdf:about="http://purl.obolibrary.org/obo/GAZ_00481095">
        <obo:RO_0001025 rdf:resource="http://purl.obolibrary.org/obo/GAZ_00481094"/>
        <obo:IAO_0000115>A lake in the High Tatras.</obo:IAO_0000115>
        <oboInOwl:hasOBONamespace>GAZ</oboInOwl:hasOBONamespace>
        <oboInOwl:id>GAZ:00481095</oboInOwl:id>
        <rdfs:label>Batizovske pleso</rdfs:label>
    </owl:NamedIndividual>
    


    <!-- http://purl.obolibrary.org/obo/GAZ_00481096 -->

    <owl:NamedIndividual rdf:about="http://purl.obolibrary.org/obo/GAZ_00481096">
        <obo:RO_0001025 rdf:resource="http://purl.obolibrary.org/obo/GAZ_00481094"/>
        <obo:IAO_0000115>A lake.</obo:IAO_0000115>
        <oboInOwl:hasOBONamespace>GAZ</oboInOwl:hasOBONamespace>
        <oboInOwl:id>GAZ:00481096</oboInOwl:id>
        <rdfs:label>Batizovske oka</rdfs:label>
    </owl:NamedIndividual>
    


    <!-- http://purl.obolibrary.org/obo/GAZ_00481097 -->

    <owl:NamedIndividual rdf:about="http://purl.obolibrary.org/obo/GAZ_00481097">
        <obo:RO_0001025 rdf:resource="http://purl.obolibrary.org/obo/GAZ_00056820"/>
        <obo:IAO_0000115>A valley.</obo:IAO_0000115>
        <oboInOwl:hasOBONamespace>GAZ</oboInOwl:hasOBONamespace>
        <oboInOwl:id>GAZ:00481097</oboInOwl:id>
        <rdfs:label>Bobrovecka dolina</rdfs:label>
    </owl:NamedIndividual>
    


    <!-- http://purl.obolibrary.org/obo/GAZ_00481098 -->

    <owl:NamedIndividual rdf:about="http://purl.obolibrary.org/obo/GAZ_00481098">
        <obo:RO_0001025 rdf:resource="http://purl.obolibrary.org/obo/GAZ_00481097"/>
        <obo:IAO_0000115>Lakes.</obo:IAO_0000115>
        <oboInOwl:hasOBONamespace>GAZ</oboInOwl:hasOBONamespace>
        <oboInOwl:id>GAZ:00481098</oboInOwl:id>
        <rdfs:label>Bobrovecke plieska</rdfs:label>
    </owl:NamedIndividual>
    


    <!-- http://purl.obolibrary.org/obo/GAZ_00481099 -->

    <owl:NamedIndividual rdf:about="http://purl.obolibrary.org/obo/GAZ_00481099">
        <obo:RO_0001025 rdf:resource="http://purl.obolibrary.org/obo/GAZ_00481098"/>
        <obo:IAO_0000115>A lake.</obo:IAO_0000115>
        <oboInOwl:hasOBONamespace>GAZ</oboInOwl:hasOBONamespace>
        <oboInOwl:id>GAZ:00481099</oboInOwl:id>
        <rdfs:label>Cierne Bobrovecke pliesko</rdfs:label>
    </owl:NamedIndividual>
    


    <!-- http://purl.obolibrary.org/obo/GAZ_00481100 -->

    <owl:NamedIndividual rdf:about="http://purl.obolibrary.org/obo/GAZ_00481100">
        <obo:RO_0001025 rdf:resource="http://purl.obolibrary.org/obo/GAZ_00481098"/>
        <obo:IAO_0000115>A lake.</obo:IAO_0000115>
        <oboInOwl:hasOBONamespace>GAZ</oboInOwl:hasOBONamespace>
        <oboInOwl:id>GAZ:00481100</oboInOwl:id>
        <rdfs:label>Male Bobrovecke pliesko</rdfs:label>
    </owl:NamedIndividual>
    


    <!-- http://purl.obolibrary.org/obo/GAZ_00481101 -->

    <owl:NamedIndividual rdf:about="http://purl.obolibrary.org/obo/GAZ_00481101">
        <obo:RO_0001025 rdf:resource="http://purl.obolibrary.org/obo/GAZ_00481098"/>
        <obo:IAO_0000115>A lake.</obo:IAO_0000115>
        <oboInOwl:hasOBONamespace>GAZ</oboInOwl:hasOBONamespace>
        <oboInOwl:id>GAZ:00481101</oboInOwl:id>
        <rdfs:label>Biele Bobrovecke pliesko</rdfs:label>
    </owl:NamedIndividual>
    


    <!-- http://purl.obolibrary.org/obo/GAZ_00481102 -->

    <owl:NamedIndividual rdf:about="http://purl.obolibrary.org/obo/GAZ_00481102">
        <obo:RO_0001025 rdf:resource="http://purl.obolibrary.org/obo/GAZ_00007974"/>
        <obo:IAO_0000115>A valley.</obo:IAO_0000115>
        <oboInOwl:hasOBONamespace>GAZ</oboInOwl:hasOBONamespace>
        <oboInOwl:id>GAZ:00481102</oboInOwl:id>
        <rdfs:label>Mlynicka dolina</rdfs:label>
    </owl:NamedIndividual>
    


    <!-- http://purl.obolibrary.org/obo/GAZ_00481103 -->

    <owl:NamedIndividual rdf:about="http://purl.obolibrary.org/obo/GAZ_00481103">
        <obo:RO_0001025 rdf:resource="http://purl.obolibrary.org/obo/GAZ_00481102"/>
        <obo:IAO_0000115>A lake.</obo:IAO_0000115>
        <oboInOwl:hasOBONamespace>GAZ</oboInOwl:hasOBONamespace>
        <oboInOwl:id>GAZ:00481103</oboInOwl:id>
        <rdfs:label>Pliesko pod Skokom</rdfs:label>
    </owl:NamedIndividual>
    


    <!-- http://purl.obolibrary.org/obo/GAZ_00481104 -->

    <owl:NamedIndividual rdf:about="http://purl.obolibrary.org/obo/GAZ_00481104">
        <obo:RO_0001025 rdf:resource="http://purl.obolibrary.org/obo/GAZ_00481102"/>
        <obo:IAO_0000115>Lakes.</obo:IAO_0000115>
        <oboInOwl:hasOBONamespace>GAZ</oboInOwl:hasOBONamespace>
        <oboInOwl:id>GAZ:00481104</oboInOwl:id>
        <rdfs:label>Volie plieska</rdfs:label>
    </owl:NamedIndividual>
    


    <!-- http://purl.obolibrary.org/obo/GAZ_00481105 -->

    <owl:NamedIndividual rdf:about="http://purl.obolibrary.org/obo/GAZ_00481105">
        <obo:RO_0001025 rdf:resource="http://purl.obolibrary.org/obo/GAZ_00481104"/>
        <obo:IAO_0000115>A lake.</obo:IAO_0000115>
        <oboInOwl:hasOBONamespace>GAZ</oboInOwl:hasOBONamespace>
        <oboInOwl:id>GAZ:00481105</oboInOwl:id>
        <rdfs:label>Nizne Volie pliesko</rdfs:label>
    </owl:NamedIndividual>
    


    <!-- http://purl.obolibrary.org/obo/GAZ_00481106 -->

    <owl:NamedIndividual rdf:about="http://purl.obolibrary.org/obo/GAZ_00481106">
        <obo:RO_0001025 rdf:resource="http://purl.obolibrary.org/obo/GAZ_00481104"/>
        <obo:IAO_0000115>A lake.</obo:IAO_0000115>
        <oboInOwl:hasOBONamespace>GAZ</oboInOwl:hasOBONamespace>
        <oboInOwl:id>GAZ:00481106</oboInOwl:id>
        <rdfs:label>Vysne Volie pliesko</rdfs:label>
    </owl:NamedIndividual>
    


    <!-- http://purl.obolibrary.org/obo/GAZ_00481107 -->

    <owl:NamedIndividual rdf:about="http://purl.obolibrary.org/obo/GAZ_00481107">
        <obo:RO_0001025 rdf:resource="http://purl.obolibrary.org/obo/GAZ_00481102"/>
        <obo:IAO_0000115>Lakes.</obo:IAO_0000115>
        <oboInOwl:hasOBONamespace>GAZ</oboInOwl:hasOBONamespace>
        <oboInOwl:id>GAZ:00481107</oboInOwl:id>
        <rdfs:label>Kozie plesa</rdfs:label>
    </owl:NamedIndividual>
    


    <!-- http://purl.obolibrary.org/obo/GAZ_00481108 -->

    <owl:NamedIndividual rdf:about="http://purl.obolibrary.org/obo/GAZ_00481108">
        <obo:RO_0001025 rdf:resource="http://purl.obolibrary.org/obo/GAZ_00481107"/>
        <obo:IAO_0000115>A lake.</obo:IAO_0000115>
        <oboInOwl:hasOBONamespace>GAZ</oboInOwl:hasOBONamespace>
        <oboInOwl:id>GAZ:00481108</oboInOwl:id>
        <rdfs:label>Vysne Kozie pleso</rdfs:label>
    </owl:NamedIndividual>
    


    <!-- http://purl.obolibrary.org/obo/GAZ_00481109 -->

    <owl:NamedIndividual rdf:about="http://purl.obolibrary.org/obo/GAZ_00481109">
        <obo:RO_0001025 rdf:resource="http://purl.obolibrary.org/obo/GAZ_00481107"/>
        <obo:IAO_0000115>A lake.</obo:IAO_0000115>
        <oboInOwl:hasOBONamespace>GAZ</oboInOwl:hasOBONamespace>
        <oboInOwl:id>GAZ:00481109</oboInOwl:id>
        <rdfs:label>Nizne Kozie pleso</rdfs:label>
    </owl:NamedIndividual>
    


    <!-- http://purl.obolibrary.org/obo/GAZ_00481110 -->

    <owl:NamedIndividual rdf:about="http://purl.obolibrary.org/obo/GAZ_00481110">
        <obo:RO_0001025 rdf:resource="http://purl.obolibrary.org/obo/GAZ_00481102"/>
        <obo:IAO_0000115>A lake.</obo:IAO_0000115>
        <oboInOwl:hasOBONamespace>GAZ</oboInOwl:hasOBONamespace>
        <oboInOwl:id>GAZ:00481110</oboInOwl:id>
        <rdfs:label>Capie pleso</rdfs:label>
    </owl:NamedIndividual>
    


    <!-- http://purl.obolibrary.org/obo/GAZ_00481111 -->

    <owl:NamedIndividual rdf:about="http://purl.obolibrary.org/obo/GAZ_00481111">
        <obo:RO_0001025 rdf:resource="http://purl.obolibrary.org/obo/GAZ_00481102"/>
        <obo:IAO_0000115>A lake.</obo:IAO_0000115>
        <oboInOwl:hasOBONamespace>GAZ</oboInOwl:hasOBONamespace>
        <oboInOwl:id>GAZ:00481111</oboInOwl:id>
        <rdfs:label>Okruhle pleso</rdfs:label>
    </owl:NamedIndividual>
    


    <!-- http://purl.obolibrary.org/obo/GAZ_00481112 -->

    <owl:NamedIndividual rdf:about="http://purl.obolibrary.org/obo/GAZ_00481112">
        <obo:RO_0001025 rdf:resource="http://purl.obolibrary.org/obo/GAZ_00007974"/>
        <obo:IAO_0000115>A valley.</obo:IAO_0000115>
        <oboInOwl:hasOBONamespace>GAZ</oboInOwl:hasOBONamespace>
        <oboInOwl:id>GAZ:00481112</oboInOwl:id>
        <rdfs:label>Siroka dolina</rdfs:label>
    </owl:NamedIndividual>
    


    <!-- http://purl.obolibrary.org/obo/GAZ_00481113 -->

    <owl:NamedIndividual rdf:about="http://purl.obolibrary.org/obo/GAZ_00481113">
        <obo:RO_0001025 rdf:resource="http://purl.obolibrary.org/obo/GAZ_00481112"/>
        <obo:IAO_0000115>A lake.</obo:IAO_0000115>
        <oboInOwl:hasOBONamespace>GAZ</oboInOwl:hasOBONamespace>
        <oboInOwl:id>GAZ:00481113</oboInOwl:id>
        <rdfs:label>Male Tiche pleso</rdfs:label>
    </owl:NamedIndividual>
    


    <!-- http://purl.obolibrary.org/obo/GAZ_00481114 -->

    <owl:NamedIndividual rdf:about="http://purl.obolibrary.org/obo/GAZ_00481114">
        <obo:RO_0001025 rdf:resource="http://purl.obolibrary.org/obo/GAZ_00481112"/>
        <obo:IAO_0000115>A lake.</obo:IAO_0000115>
        <oboInOwl:hasOBONamespace>GAZ</oboInOwl:hasOBONamespace>
        <oboInOwl:id>GAZ:00481114</oboInOwl:id>
        <rdfs:label>Tiche pleso</rdfs:label>
    </owl:NamedIndividual>
    


    <!-- http://purl.obolibrary.org/obo/GAZ_00481115 -->

    <owl:NamedIndividual rdf:about="http://purl.obolibrary.org/obo/GAZ_00481115">
        <obo:RO_0001025 rdf:resource="http://purl.obolibrary.org/obo/GAZ_00007974"/>
        <obo:IAO_0000115>A valley.</obo:IAO_0000115>
        <oboInOwl:hasOBONamespace>GAZ</oboInOwl:hasOBONamespace>
        <oboInOwl:id>GAZ:00481115</oboInOwl:id>
        <rdfs:label>Tazka dolina</rdfs:label>
    </owl:NamedIndividual>
    


    <!-- http://purl.obolibrary.org/obo/GAZ_00481116 -->

    <owl:NamedIndividual rdf:about="http://purl.obolibrary.org/obo/GAZ_00481116">
        <obo:RO_0001025 rdf:resource="http://purl.obolibrary.org/obo/GAZ_00481115"/>
        <obo:IAO_0000115>A lake in the High Tatras.</obo:IAO_0000115>
        <oboInOwl:hasOBONamespace>GAZ</oboInOwl:hasOBONamespace>
        <oboInOwl:id>GAZ:00481116</oboInOwl:id>
        <rdfs:label>Tazke pleso</rdfs:label>
    </owl:NamedIndividual>
    


    <!-- http://purl.obolibrary.org/obo/GAZ_00481117 -->

    <owl:NamedIndividual rdf:about="http://purl.obolibrary.org/obo/GAZ_00481117">
        <obo:RO_0001025 rdf:resource="http://purl.obolibrary.org/obo/GAZ_00056820"/>
        <obo:IAO_0000115>A valley.</obo:IAO_0000115>
        <oboInOwl:hasOBONamespace>GAZ</oboInOwl:hasOBONamespace>
        <oboInOwl:id>GAZ:00481117</oboInOwl:id>
        <rdfs:label>Studena dolina</rdfs:label>
    </owl:NamedIndividual>
    


    <!-- http://purl.obolibrary.org/obo/GAZ_00481119 -->

    <owl:NamedIndividual rdf:about="http://purl.obolibrary.org/obo/GAZ_00481119">
        <obo:IAO_0000115>A lake.</obo:IAO_0000115>
        <oboInOwl:hasOBONamespace>GAZ</oboInOwl:hasOBONamespace>
        <oboInOwl:id>GAZ:00481119</oboInOwl:id>
        <rdfs:label>Cierna mlaka</rdfs:label>
    </owl:NamedIndividual>
    


    <!-- http://purl.obolibrary.org/obo/GAZ_00481120 -->

    <owl:NamedIndividual rdf:about="http://purl.obolibrary.org/obo/GAZ_00481120">
        <obo:RO_0001025 rdf:resource="http://purl.obolibrary.org/obo/GAZ_00481094"/>
        <obo:IAO_0000115>A lake.</obo:IAO_0000115>
        <oboInOwl:hasOBONamespace>GAZ</oboInOwl:hasOBONamespace>
        <oboInOwl:id>GAZ:00481120</oboInOwl:id>
        <rdfs:label>Cierne pleso</rdfs:label>
    </owl:NamedIndividual>
    


    <!-- http://purl.obolibrary.org/obo/GAZ_00481121 -->

    <owl:NamedIndividual rdf:about="http://purl.obolibrary.org/obo/GAZ_00481121">
        <obo:RO_0001025 rdf:resource="http://purl.obolibrary.org/obo/GAZ_00007974"/>
        <obo:IAO_0000115>A valley.</obo:IAO_0000115>
        <oboInOwl:hasOBONamespace>GAZ</oboInOwl:hasOBONamespace>
        <oboInOwl:id>GAZ:00481121</oboInOwl:id>
        <rdfs:label>Javorova dolina</rdfs:label>
    </owl:NamedIndividual>
    


    <!-- http://purl.obolibrary.org/obo/GAZ_00481123 -->

    <owl:NamedIndividual rdf:about="http://purl.obolibrary.org/obo/GAZ_00481123">
        <obo:IAO_0000115>A lake.</obo:IAO_0000115>
        <oboInOwl:hasOBONamespace>GAZ</oboInOwl:hasOBONamespace>
        <oboInOwl:id>GAZ:00481123</oboInOwl:id>
        <rdfs:label>Cierne Javorove pleso</rdfs:label>
    </owl:NamedIndividual>
    


    <!-- http://purl.obolibrary.org/obo/GAZ_00481124 -->

    <owl:NamedIndividual rdf:about="http://purl.obolibrary.org/obo/GAZ_00481124">
        <obo:RO_0001025 rdf:resource="http://purl.obolibrary.org/obo/GAZ_00007974"/>
        <obo:IAO_0000115>A valley.</obo:IAO_0000115>
        <oboInOwl:hasOBONamespace>GAZ</oboInOwl:hasOBONamespace>
        <oboInOwl:id>GAZ:00481124</oboInOwl:id>
        <rdfs:label>Dolina Bielej vody Kezmarskej</rdfs:label>
    </owl:NamedIndividual>
    


    <!-- http://purl.obolibrary.org/obo/GAZ_00481126 -->

    <owl:NamedIndividual rdf:about="http://purl.obolibrary.org/obo/GAZ_00481126">
        <obo:IAO_0000115>A lake.</obo:IAO_0000115>
        <oboInOwl:hasOBONamespace>GAZ</oboInOwl:hasOBONamespace>
        <oboInOwl:id>GAZ:00481126</oboInOwl:id>
        <rdfs:label>Cierne pleso Kezmarske</rdfs:label>
    </owl:NamedIndividual>
    


    <!-- http://purl.obolibrary.org/obo/GAZ_00481127 -->

    <owl:NamedIndividual rdf:about="http://purl.obolibrary.org/obo/GAZ_00481127">
        <obo:IAO_0000115>A valley.</obo:IAO_0000115>
        <oboInOwl:hasOBONamespace>GAZ</oboInOwl:hasOBONamespace>
        <oboInOwl:id>GAZ:00481127</oboInOwl:id>
        <rdfs:label>Cervena dolina</rdfs:label>
    </owl:NamedIndividual>
    


    <!-- http://purl.obolibrary.org/obo/GAZ_00481128 -->

    <owl:NamedIndividual rdf:about="http://purl.obolibrary.org/obo/GAZ_00481128">
        <obo:RO_0001025 rdf:resource="http://purl.obolibrary.org/obo/GAZ_00481127"/>
        <obo:IAO_0000115>A lake.</obo:IAO_0000115>
        <oboInOwl:hasOBONamespace>GAZ</oboInOwl:hasOBONamespace>
        <oboInOwl:id>GAZ:00481128</oboInOwl:id>
        <rdfs:label>Kezmarske Cervene pleso</rdfs:label>
    </owl:NamedIndividual>
    


    <!-- http://purl.obolibrary.org/obo/GAZ_00481129 -->

    <owl:NamedIndividual rdf:about="http://purl.obolibrary.org/obo/GAZ_00481129">
        <obo:RO_0001025 rdf:resource="http://purl.obolibrary.org/obo/GAZ_00481127"/>
        <obo:IAO_0000115>A lake.</obo:IAO_0000115>
        <oboInOwl:hasOBONamespace>GAZ</oboInOwl:hasOBONamespace>
        <oboInOwl:id>GAZ:00481129</oboInOwl:id>
        <rdfs:label>Belase pleso</rdfs:label>
    </owl:NamedIndividual>
    


    <!-- http://purl.obolibrary.org/obo/GAZ_00481130 -->

    <owl:NamedIndividual rdf:about="http://purl.obolibrary.org/obo/GAZ_00481130">
        <obo:RO_0001025 rdf:resource="http://purl.obolibrary.org/obo/GAZ_00481127"/>
        <obo:IAO_0000115>A lake.</obo:IAO_0000115>
        <oboInOwl:hasOBONamespace>GAZ</oboInOwl:hasOBONamespace>
        <oboInOwl:id>GAZ:00481130</oboInOwl:id>
        <rdfs:label>Male Cervene pliesko</rdfs:label>
    </owl:NamedIndividual>
    


    <!-- http://purl.obolibrary.org/obo/GAZ_00481131 -->

    <owl:NamedIndividual rdf:about="http://purl.obolibrary.org/obo/GAZ_00481131">
        <obo:RO_0001025 rdf:resource="http://purl.obolibrary.org/obo/GAZ_00007974"/>
        <obo:IAO_0000115>A valley.</obo:IAO_0000115>
        <oboInOwl:hasOBONamespace>GAZ</oboInOwl:hasOBONamespace>
        <oboInOwl:id>GAZ:00481131</oboInOwl:id>
        <rdfs:label>Studena dolina</rdfs:label>
    </owl:NamedIndividual>
    


    <!-- http://purl.obolibrary.org/obo/GAZ_00481133 -->

    <owl:NamedIndividual rdf:about="http://purl.obolibrary.org/obo/GAZ_00481133">
        <obo:IAO_0000115>A lake.</obo:IAO_0000115>
        <oboInOwl:hasOBONamespace>GAZ</oboInOwl:hasOBONamespace>
        <oboInOwl:id>GAZ:00481133</oboInOwl:id>
        <rdfs:label>Vareskove pleso</rdfs:label>
    </owl:NamedIndividual>
    


    <!-- http://purl.obolibrary.org/obo/GAZ_00481134 -->

    <owl:NamedIndividual rdf:about="http://purl.obolibrary.org/obo/GAZ_00481134">
        <obo:IAO_0000115>A lake.</obo:IAO_0000115>
        <oboInOwl:hasOBONamespace>GAZ</oboInOwl:hasOBONamespace>
        <oboInOwl:id>GAZ:00481134</oboInOwl:id>
        <rdfs:label>Dlhe pleso</rdfs:label>
    </owl:NamedIndividual>
    


    <!-- http://purl.obolibrary.org/obo/GAZ_00481135 -->

    <owl:NamedIndividual rdf:about="http://purl.obolibrary.org/obo/GAZ_00481135">
        <obo:IAO_0000115>A lake.</obo:IAO_0000115>
        <oboInOwl:hasOBONamespace>GAZ</oboInOwl:hasOBONamespace>
        <oboInOwl:id>GAZ:00481135</oboInOwl:id>
        <rdfs:label>Starolesnianske pleso</rdfs:label>
    </owl:NamedIndividual>
    


    <!-- http://purl.obolibrary.org/obo/GAZ_00481137 -->

    <owl:NamedIndividual rdf:about="http://purl.obolibrary.org/obo/GAZ_00481137">
        <obo:IAO_0000115>A lake.</obo:IAO_0000115>
        <oboInOwl:hasOBONamespace>GAZ</oboInOwl:hasOBONamespace>
        <oboInOwl:id>GAZ:00481137</oboInOwl:id>
        <rdfs:label>Puste Puste pleso</rdfs:label>
    </owl:NamedIndividual>
    


    <!-- http://purl.obolibrary.org/obo/GAZ_00481138 -->

    <owl:NamedIndividual rdf:about="http://purl.obolibrary.org/obo/GAZ_00481138">
        <obo:IAO_0000115>A lake.</obo:IAO_0000115>
        <oboInOwl:hasOBONamespace>GAZ</oboInOwl:hasOBONamespace>
        <oboInOwl:id>GAZ:00481138</oboInOwl:id>
        <rdfs:label>Male Puste pleso</rdfs:label>
    </owl:NamedIndividual>
    


    <!-- http://purl.obolibrary.org/obo/GAZ_00481139 -->

    <owl:NamedIndividual rdf:about="http://purl.obolibrary.org/obo/GAZ_00481139">
        <obo:IAO_0000115>Lakes.</obo:IAO_0000115>
        <oboInOwl:hasOBONamespace>GAZ</oboInOwl:hasOBONamespace>
        <oboInOwl:id>GAZ:00481139</oboInOwl:id>
        <rdfs:label>Vysne Strelecke plesa</rdfs:label>
    </owl:NamedIndividual>
    


    <!-- http://purl.obolibrary.org/obo/GAZ_00481140 -->

    <owl:NamedIndividual rdf:about="http://purl.obolibrary.org/obo/GAZ_00481140">
        <obo:IAO_0000115>Lakes.</obo:IAO_0000115>
        <oboInOwl:hasOBONamespace>GAZ</oboInOwl:hasOBONamespace>
        <oboInOwl:id>GAZ:00481140</oboInOwl:id>
        <rdfs:label>Sive plesa</rdfs:label>
    </owl:NamedIndividual>
    


    <!-- http://purl.obolibrary.org/obo/GAZ_00481141 -->

    <owl:NamedIndividual rdf:about="http://purl.obolibrary.org/obo/GAZ_00481141">
        <obo:IAO_0000115>A lake.</obo:IAO_0000115>
        <oboInOwl:hasOBONamespace>GAZ</oboInOwl:hasOBONamespace>
        <oboInOwl:id>GAZ:00481141</oboInOwl:id>
        <rdfs:label>Studene plesa</rdfs:label>
    </owl:NamedIndividual>
    


    <!-- http://purl.obolibrary.org/obo/GAZ_00481142 -->

    <owl:NamedIndividual rdf:about="http://purl.obolibrary.org/obo/GAZ_00481142">
        <obo:IAO_0000115>A lake.</obo:IAO_0000115>
        <oboInOwl:hasOBONamespace>GAZ</oboInOwl:hasOBONamespace>
        <oboInOwl:id>GAZ:00481142</oboInOwl:id>
        <rdfs:label>Nizne Strelecke plesa</rdfs:label>
    </owl:NamedIndividual>
    


    <!-- http://purl.obolibrary.org/obo/GAZ_00481143 -->

    <owl:NamedIndividual rdf:about="http://purl.obolibrary.org/obo/GAZ_00481143">
        <obo:IAO_0000115>Lakes.</obo:IAO_0000115>
        <oboInOwl:hasOBONamespace>GAZ</oboInOwl:hasOBONamespace>
        <oboInOwl:id>GAZ:00481143</oboInOwl:id>
        <rdfs:label>Sesterske plesa</rdfs:label>
    </owl:NamedIndividual>
    


    <!-- http://purl.obolibrary.org/obo/GAZ_00481145 -->

    <owl:NamedIndividual rdf:about="http://purl.obolibrary.org/obo/GAZ_00481145">
        <obo:IAO_0000115>A lake.</obo:IAO_0000115>
        <oboInOwl:hasOBONamespace>GAZ</oboInOwl:hasOBONamespace>
        <oboInOwl:id>GAZ:00481145</oboInOwl:id>
        <rdfs:label>Zbojnicke plesa</rdfs:label>
    </owl:NamedIndividual>
    


    <!-- http://purl.obolibrary.org/obo/GAZ_00481146 -->

    <owl:NamedIndividual rdf:about="http://purl.obolibrary.org/obo/GAZ_00481146">
        <obo:RO_0001025 rdf:resource="http://purl.obolibrary.org/obo/GAZ_00007974"/>
        <obo:IAO_0000115>A valley.</obo:IAO_0000115>
        <oboInOwl:hasOBONamespace>GAZ</oboInOwl:hasOBONamespace>
        <oboInOwl:id>GAZ:00481146</oboInOwl:id>
        <rdfs:label>Velicka dolina</rdfs:label>
    </owl:NamedIndividual>
    


    <!-- http://purl.obolibrary.org/obo/GAZ_00481147 -->

    <owl:NamedIndividual rdf:about="http://purl.obolibrary.org/obo/GAZ_00481147">
        <obo:RO_0001025 rdf:resource="http://purl.obolibrary.org/obo/GAZ_00481146"/>
        <obo:IAO_0000115>A lake.</obo:IAO_0000115>
        <oboInOwl:hasOBONamespace>GAZ</oboInOwl:hasOBONamespace>
        <oboInOwl:id>GAZ:00481147</oboInOwl:id>
        <rdfs:label>Dlhe pleso Velicke</rdfs:label>
    </owl:NamedIndividual>
    


    <!-- http://purl.obolibrary.org/obo/GAZ_00481148 -->

    <owl:NamedIndividual rdf:about="http://purl.obolibrary.org/obo/GAZ_00481148">
        <obo:RO_0001025 rdf:resource="http://purl.obolibrary.org/obo/GAZ_00007974"/>
        <obo:IAO_0000115>A valley.</obo:IAO_0000115>
        <oboInOwl:hasOBONamespace>GAZ</oboInOwl:hasOBONamespace>
        <oboInOwl:id>GAZ:00481148</oboInOwl:id>
        <rdfs:label>Dolina Suchej Wody Gasienicowej</rdfs:label>
    </owl:NamedIndividual>
    


    <!-- http://purl.obolibrary.org/obo/GAZ_00481150 -->

    <owl:NamedIndividual rdf:about="http://purl.obolibrary.org/obo/GAZ_00481150">
        <obo:RO_0001025 rdf:resource="http://purl.obolibrary.org/obo/GAZ_00007974"/>
        <obo:IAO_0000115>A valley.</obo:IAO_0000115>
        <oboInOwl:hasOBONamespace>GAZ</oboInOwl:hasOBONamespace>
        <oboInOwl:id>GAZ:00481150</oboInOwl:id>
        <rdfs:label>Dolina Bialki</rdfs:label>
    </owl:NamedIndividual>
    


    <!-- http://purl.obolibrary.org/obo/GAZ_00481160 -->

    <owl:NamedIndividual rdf:about="http://purl.obolibrary.org/obo/GAZ_00481160">
        <obo:RO_0001025 rdf:resource="http://purl.obolibrary.org/obo/GAZ_00056821"/>
        <obo:IAO_0000115>A valley.</obo:IAO_0000115>
        <oboInOwl:hasOBONamespace>GAZ</oboInOwl:hasOBONamespace>
        <oboInOwl:id>GAZ:00481160</oboInOwl:id>
        <rdfs:label>Dolina Kezmarskej Bielej vody</rdfs:label>
    </owl:NamedIndividual>
    


    <!-- http://purl.obolibrary.org/obo/GAZ_00481164 -->

    <owl:NamedIndividual rdf:about="http://purl.obolibrary.org/obo/GAZ_00481164">
        <obo:IAO_0000115>A lake.</obo:IAO_0000115>
        <oboInOwl:hasOBONamespace>GAZ</oboInOwl:hasOBONamespace>
        <oboInOwl:id>GAZ:00481164</oboInOwl:id>
        <rdfs:label>Trojuholnikove pleso</rdfs:label>
    </owl:NamedIndividual>
    


    <!-- http://purl.obolibrary.org/obo/GAZ_00481165 -->

    <owl:NamedIndividual rdf:about="http://purl.obolibrary.org/obo/GAZ_00481165">
        <obo:IAO_0000115>A lake.</obo:IAO_0000115>
        <oboInOwl:hasOBONamespace>GAZ</oboInOwl:hasOBONamespace>
        <oboInOwl:id>GAZ:00481165</oboInOwl:id>
        <rdfs:label>Male Biele plesa</rdfs:label>
    </owl:NamedIndividual>
    


    <!-- http://purl.obolibrary.org/obo/GAZ_00481166 -->

    <owl:NamedIndividual rdf:about="http://purl.obolibrary.org/obo/GAZ_00481166">
        <obo:IAO_0000115>A lake.</obo:IAO_0000115>
        <oboInOwl:hasOBONamespace>GAZ</oboInOwl:hasOBONamespace>
        <oboInOwl:id>GAZ:00481166</oboInOwl:id>
        <rdfs:label>Nizne Zeruchove pliesko</rdfs:label>
    </owl:NamedIndividual>
    


    <!-- http://purl.obolibrary.org/obo/GAZ_00481167 -->

    <owl:NamedIndividual rdf:about="http://purl.obolibrary.org/obo/GAZ_00481167">
        <obo:IAO_0000115>A lake.</obo:IAO_0000115>
        <oboInOwl:hasOBONamespace>GAZ</oboInOwl:hasOBONamespace>
        <oboInOwl:id>GAZ:00481167</oboInOwl:id>
        <rdfs:label>Vysne Zeruchove pliesko</rdfs:label>
    </owl:NamedIndividual>
    


    <!-- http://purl.obolibrary.org/obo/GAZ_00481168 -->

    <owl:NamedIndividual rdf:about="http://purl.obolibrary.org/obo/GAZ_00481168">
        <obo:IAO_0000115>A lake.</obo:IAO_0000115>
        <oboInOwl:hasOBONamespace>GAZ</oboInOwl:hasOBONamespace>
        <oboInOwl:id>GAZ:00481168</oboInOwl:id>
        <rdfs:label>Zlte pleso</rdfs:label>
    </owl:NamedIndividual>
    


    <!-- http://purl.obolibrary.org/obo/GAZ_00481173 -->

    <owl:NamedIndividual rdf:about="http://purl.obolibrary.org/obo/GAZ_00481173">
        <obo:IAO_0000115>A lake.</obo:IAO_0000115>
        <oboInOwl:hasOBONamespace>GAZ</oboInOwl:hasOBONamespace>
        <oboInOwl:id>GAZ:00481173</oboInOwl:id>
        <rdfs:label>Vel&apos;ke spisske pleso</rdfs:label>
    </owl:NamedIndividual>
    


    <!-- http://purl.obolibrary.org/obo/GAZ_00481174 -->

    <owl:NamedIndividual rdf:about="http://purl.obolibrary.org/obo/GAZ_00481174">
        <obo:IAO_0000115>A lake.</obo:IAO_0000115>
        <oboInOwl:hasOBONamespace>GAZ</oboInOwl:hasOBONamespace>
        <oboInOwl:id>GAZ:00481174</oboInOwl:id>
        <rdfs:label>Prostredne spisske pleso</rdfs:label>
    </owl:NamedIndividual>
    


    <!-- http://purl.obolibrary.org/obo/GAZ_00481175 -->

    <owl:NamedIndividual rdf:about="http://purl.obolibrary.org/obo/GAZ_00481175">
        <obo:IAO_0000115>A lake.</obo:IAO_0000115>
        <oboInOwl:hasOBONamespace>GAZ</oboInOwl:hasOBONamespace>
        <oboInOwl:id>GAZ:00481175</oboInOwl:id>
        <rdfs:label>Nizne spisske pleso</rdfs:label>
    </owl:NamedIndividual>
    


    <!-- http://purl.obolibrary.org/obo/GAZ_00481176 -->

    <owl:NamedIndividual rdf:about="http://purl.obolibrary.org/obo/GAZ_00481176">
        <obo:IAO_0000115>A lake.</obo:IAO_0000115>
        <oboInOwl:hasOBONamespace>GAZ</oboInOwl:hasOBONamespace>
        <oboInOwl:id>GAZ:00481176</oboInOwl:id>
        <rdfs:label>Vysne spisske pleso</rdfs:label>
    </owl:NamedIndividual>
    


    <!-- http://purl.obolibrary.org/obo/GAZ_00481177 -->

    <owl:NamedIndividual rdf:about="http://purl.obolibrary.org/obo/GAZ_00481177">
        <obo:IAO_0000115>A lake.</obo:IAO_0000115>
        <oboInOwl:hasOBONamespace>GAZ</oboInOwl:hasOBONamespace>
        <oboInOwl:id>GAZ:00481177</oboInOwl:id>
        <rdfs:label>Male spisske pleso</rdfs:label>
    </owl:NamedIndividual>
    


    <!-- http://purl.obolibrary.org/obo/GAZ_00481178 -->

    <owl:NamedIndividual rdf:about="http://purl.obolibrary.org/obo/GAZ_00481178">
        <obo:RO_0001025 rdf:resource="http://purl.obolibrary.org/obo/GAZ_00007974"/>
        <obo:IAO_0000115>A valley.</obo:IAO_0000115>
        <oboInOwl:hasOBONamespace>GAZ</oboInOwl:hasOBONamespace>
        <oboInOwl:id>GAZ:00481178</oboInOwl:id>
        <rdfs:label>Mengusovska dolina</rdfs:label>
    </owl:NamedIndividual>
    


    <!-- http://purl.obolibrary.org/obo/GAZ_00481182 -->

    <owl:NamedIndividual rdf:about="http://purl.obolibrary.org/obo/GAZ_00481182">
        <obo:IAO_0000115>A lake.</obo:IAO_0000115>
        <oboInOwl:hasOBONamespace>GAZ</oboInOwl:hasOBONamespace>
        <oboInOwl:id>GAZ:00481182</oboInOwl:id>
        <rdfs:label>Male Hincovo pleso</rdfs:label>
    </owl:NamedIndividual>
    


    <!-- http://purl.obolibrary.org/obo/GAZ_00481183 -->

    <owl:NamedIndividual rdf:about="http://purl.obolibrary.org/obo/GAZ_00481183">
        <obo:RO_0001025 rdf:resource="http://purl.obolibrary.org/obo/GAZ_00007974"/>
        <obo:IAO_0000115>A valley.</obo:IAO_0000115>
        <oboInOwl:hasOBONamespace>GAZ</oboInOwl:hasOBONamespace>
        <oboInOwl:id>GAZ:00481183</oboInOwl:id>
        <rdfs:label>Furkotska dolina</rdfs:label>
    </owl:NamedIndividual>
    


    <!-- http://purl.obolibrary.org/obo/GAZ_00481184 -->

    <owl:NamedIndividual rdf:about="http://purl.obolibrary.org/obo/GAZ_00481184">
        <obo:RO_0001025 rdf:resource="http://purl.obolibrary.org/obo/GAZ_00007974"/>
        <obo:IAO_0000115>A lake of glacial origin in the High Tatras in the settlement Strbske Pleso in Slovakia.</obo:IAO_0000115>
        <oboInOwl:hasOBONamespace>GAZ</oboInOwl:hasOBONamespace>
        <oboInOwl:id>GAZ:00481184</oboInOwl:id>
        <rdfs:label>Strbske Pleso</rdfs:label>
    </owl:NamedIndividual>
    


    <!-- http://purl.obolibrary.org/obo/GAZ_00481185 -->

    <owl:NamedIndividual rdf:about="http://purl.obolibrary.org/obo/GAZ_00481185">
        <obo:RO_0001025 rdf:resource="http://purl.obolibrary.org/obo/GAZ_00481183"/>
        <obo:IAO_0000115>A lake.</obo:IAO_0000115>
        <oboInOwl:hasOBONamespace>GAZ</oboInOwl:hasOBONamespace>
        <oboInOwl:id>GAZ:00481185</oboInOwl:id>
        <rdfs:label>Nizne Wahlenbergovo pleso</rdfs:label>
    </owl:NamedIndividual>
    


    <!-- http://purl.obolibrary.org/obo/GAZ_00481186 -->

    <owl:NamedIndividual rdf:about="http://purl.obolibrary.org/obo/GAZ_00481186">
        <obo:RO_0001025 rdf:resource="http://purl.obolibrary.org/obo/GAZ_00481183"/>
        <obo:IAO_0000115>Lakes.</obo:IAO_0000115>
        <oboInOwl:hasOBONamespace>GAZ</oboInOwl:hasOBONamespace>
        <oboInOwl:id>GAZ:00481186</oboInOwl:id>
        <rdfs:label>Soliskove pliesko</rdfs:label>
    </owl:NamedIndividual>
    


    <!-- http://purl.obolibrary.org/obo/GAZ_00481187 -->

    <owl:NamedIndividual rdf:about="http://purl.obolibrary.org/obo/GAZ_00481187">
        <obo:RO_0001025 rdf:resource="http://purl.obolibrary.org/obo/GAZ_00007974"/>
        <obo:IAO_0000115>A valley.</obo:IAO_0000115>
        <oboInOwl:hasOBONamespace>GAZ</oboInOwl:hasOBONamespace>
        <oboInOwl:id>GAZ:00481187</oboInOwl:id>
        <rdfs:label>Koprova dolina</rdfs:label>
    </owl:NamedIndividual>
    


    <!-- http://purl.obolibrary.org/obo/GAZ_00481191 -->

    <owl:NamedIndividual rdf:about="http://purl.obolibrary.org/obo/GAZ_00481191">
        <obo:RO_0001025 rdf:resource="http://purl.obolibrary.org/obo/GAZ_00007974"/>
        <obo:IAO_0000115>A valley.</obo:IAO_0000115>
        <oboInOwl:hasOBONamespace>GAZ</oboInOwl:hasOBONamespace>
        <oboInOwl:id>GAZ:00481191</oboInOwl:id>
        <rdfs:label>Ticha dolina</rdfs:label>
    </owl:NamedIndividual>
    


    <!-- http://purl.obolibrary.org/obo/GAZ_00481192 -->

    <owl:NamedIndividual rdf:about="http://purl.obolibrary.org/obo/GAZ_00481192">
        <obo:IAO_0000115>A lake.</obo:IAO_0000115>
        <oboInOwl:hasOBONamespace>GAZ</oboInOwl:hasOBONamespace>
        <oboInOwl:id>GAZ:00481192</oboInOwl:id>
        <rdfs:label>Dlhe oko</rdfs:label>
    </owl:NamedIndividual>
    


    <!-- http://purl.obolibrary.org/obo/GAZ_00481193 -->

    <owl:NamedIndividual rdf:about="http://purl.obolibrary.org/obo/GAZ_00481193">
        <obo:RO_0001025 rdf:resource="http://purl.obolibrary.org/obo/GAZ_00056820"/>
        <obo:IAO_0000115>A valley; on the Polish side of the Western Tatras.</obo:IAO_0000115>
        <oboInOwl:hasOBONamespace>GAZ</oboInOwl:hasOBONamespace>
        <oboInOwl:id>GAZ:00481193</oboInOwl:id>
        <rdfs:label>Dolina Olczyska</rdfs:label>
    </owl:NamedIndividual>
    


    <!-- http://purl.obolibrary.org/obo/GAZ_00481194 -->

    <owl:NamedIndividual rdf:about="http://purl.obolibrary.org/obo/GAZ_00481194">
        <obo:RO_0001025 rdf:resource="http://purl.obolibrary.org/obo/GAZ_00056820"/>
        <obo:IAO_0000115>A valley; on the Polish side of the Western Tatras.</obo:IAO_0000115>
        <oboInOwl:hasOBONamespace>GAZ</oboInOwl:hasOBONamespace>
        <oboInOwl:id>GAZ:00481194</oboInOwl:id>
        <rdfs:label>Dolina Bystrej</rdfs:label>
    </owl:NamedIndividual>
    


    <!-- http://purl.obolibrary.org/obo/GAZ_00481197 -->

    <owl:NamedIndividual rdf:about="http://purl.obolibrary.org/obo/GAZ_00481197">
        <obo:RO_0001025 rdf:resource="http://purl.obolibrary.org/obo/GAZ_00056820"/>
        <obo:IAO_0000115>A valley; on the Polish side of the Western Tatras.</obo:IAO_0000115>
        <oboInOwl:hasOBONamespace>GAZ</oboInOwl:hasOBONamespace>
        <oboInOwl:id>GAZ:00481197</oboInOwl:id>
        <rdfs:label>Dolina Bialego</rdfs:label>
    </owl:NamedIndividual>
    


    <!-- http://purl.obolibrary.org/obo/GAZ_00481198 -->

    <owl:NamedIndividual rdf:about="http://purl.obolibrary.org/obo/GAZ_00481198">
        <obo:RO_0001025 rdf:resource="http://purl.obolibrary.org/obo/GAZ_00056820"/>
        <obo:IAO_0000115>A valley; on the Polish side of the Western Tatras.</obo:IAO_0000115>
        <oboInOwl:hasOBONamespace>GAZ</oboInOwl:hasOBONamespace>
        <oboInOwl:id>GAZ:00481198</oboInOwl:id>
        <rdfs:label>Dolina ku Dziurze</rdfs:label>
    </owl:NamedIndividual>
    


    <!-- http://purl.obolibrary.org/obo/GAZ_00481199 -->

    <owl:NamedIndividual rdf:about="http://purl.obolibrary.org/obo/GAZ_00481199">
        <obo:RO_0001025 rdf:resource="http://purl.obolibrary.org/obo/GAZ_00056820"/>
        <obo:IAO_0000115>A valley; on the Polish side of the Western Tatras.</obo:IAO_0000115>
        <oboInOwl:hasOBONamespace>GAZ</oboInOwl:hasOBONamespace>
        <oboInOwl:id>GAZ:00481199</oboInOwl:id>
        <rdfs:label>Dolina Strazyska</rdfs:label>
    </owl:NamedIndividual>
    


    <!-- http://purl.obolibrary.org/obo/GAZ_00481200 -->

    <owl:NamedIndividual rdf:about="http://purl.obolibrary.org/obo/GAZ_00481200">
        <obo:RO_0001025 rdf:resource="http://purl.obolibrary.org/obo/GAZ_00056820"/>
        <obo:IAO_0000115>A valley; on the Polish side of the Western Tatras.</obo:IAO_0000115>
        <oboInOwl:hasOBONamespace>GAZ</oboInOwl:hasOBONamespace>
        <oboInOwl:id>GAZ:00481200</oboInOwl:id>
        <rdfs:label>Dolina za Bramka</rdfs:label>
    </owl:NamedIndividual>
    


    <!-- http://purl.obolibrary.org/obo/GAZ_00481201 -->

    <owl:NamedIndividual rdf:about="http://purl.obolibrary.org/obo/GAZ_00481201">
        <obo:RO_0001025 rdf:resource="http://purl.obolibrary.org/obo/GAZ_00056820"/>
        <obo:IAO_0000115>A valley; on the Polish side of the Western Tatras.</obo:IAO_0000115>
        <oboInOwl:hasOBONamespace>GAZ</oboInOwl:hasOBONamespace>
        <oboInOwl:id>GAZ:00481201</oboInOwl:id>
        <rdfs:label>Dolina Malej Laki</rdfs:label>
    </owl:NamedIndividual>
    


    <!-- http://purl.obolibrary.org/obo/GAZ_00481203 -->

    <owl:NamedIndividual rdf:about="http://purl.obolibrary.org/obo/GAZ_00481203">
        <obo:RO_0001025 rdf:resource="http://purl.obolibrary.org/obo/GAZ_00481061"/>
        <obo:IAO_0000115>A valley; on the Polish side of the Western Tatras.</obo:IAO_0000115>
        <oboInOwl:hasOBONamespace>GAZ</oboInOwl:hasOBONamespace>
        <oboInOwl:id>GAZ:00481203</oboInOwl:id>
        <rdfs:label>Dolina Tomanowa</rdfs:label>
    </owl:NamedIndividual>
    


    <!-- http://purl.obolibrary.org/obo/GAZ_00481204 -->

    <owl:NamedIndividual rdf:about="http://purl.obolibrary.org/obo/GAZ_00481204">
        <obo:RO_0001025 rdf:resource="http://purl.obolibrary.org/obo/GAZ_00056820"/>
        <obo:IAO_0000115>A valley; on the Polish side of the Western Tatras.</obo:IAO_0000115>
        <oboInOwl:hasOBONamespace>GAZ</oboInOwl:hasOBONamespace>
        <oboInOwl:id>GAZ:00481204</oboInOwl:id>
        <rdfs:label>Dolina Lejowa</rdfs:label>
    </owl:NamedIndividual>
    


    <!-- http://purl.obolibrary.org/obo/GAZ_00481208 -->

    <owl:NamedIndividual rdf:about="http://purl.obolibrary.org/obo/GAZ_00481208">
        <obo:RO_0001025 rdf:resource="http://purl.obolibrary.org/obo/GAZ_00056820"/>
        <obo:IAO_0000115>A valley; on the Slovak side of the Western Tatras.</obo:IAO_0000115>
        <oboInOwl:hasOBONamespace>GAZ</oboInOwl:hasOBONamespace>
        <oboInOwl:id>GAZ:00481208</oboInOwl:id>
        <rdfs:label>Jalovska dolina</rdfs:label>
    </owl:NamedIndividual>
    


    <!-- http://purl.obolibrary.org/obo/GAZ_00481209 -->

    <owl:NamedIndividual rdf:about="http://purl.obolibrary.org/obo/GAZ_00481209">
        <obo:RO_0001025 rdf:resource="http://purl.obolibrary.org/obo/GAZ_00056820"/>
        <obo:IAO_0000115>A valley.</obo:IAO_0000115>
        <oboInOwl:hasOBONamespace>GAZ</oboInOwl:hasOBONamespace>
        <oboInOwl:id>GAZ:00481209</oboInOwl:id>
        <rdfs:label>Gaborova dolina</rdfs:label>
    </owl:NamedIndividual>
    


    <!-- http://purl.obolibrary.org/obo/GAZ_00481210 -->

    <owl:NamedIndividual rdf:about="http://purl.obolibrary.org/obo/GAZ_00481210">
        <obo:RO_0001025 rdf:resource="http://purl.obolibrary.org/obo/GAZ_00056820"/>
        <obo:IAO_0000115>A valley; on the Slovak side of the Western Tatras.</obo:IAO_0000115>
        <oboInOwl:hasOBONamespace>GAZ</oboInOwl:hasOBONamespace>
        <oboInOwl:id>GAZ:00481210</oboInOwl:id>
        <rdfs:label>Ziarska dolina</rdfs:label>
    </owl:NamedIndividual>
    


    <!-- http://purl.obolibrary.org/obo/GAZ_00481211 -->

    <owl:NamedIndividual rdf:about="http://purl.obolibrary.org/obo/GAZ_00481211">
        <obo:RO_0001025 rdf:resource="http://purl.obolibrary.org/obo/GAZ_00056820"/>
        <obo:IAO_0000115>A valley; on the Slovak side of the Western Tatras.</obo:IAO_0000115>
        <oboInOwl:hasOBONamespace>GAZ</oboInOwl:hasOBONamespace>
        <oboInOwl:id>GAZ:00481211</oboInOwl:id>
        <rdfs:label>Jamnicka dolina</rdfs:label>
    </owl:NamedIndividual>
    


    <!-- http://purl.obolibrary.org/obo/GAZ_00481212 -->

    <owl:NamedIndividual rdf:about="http://purl.obolibrary.org/obo/GAZ_00481212">
        <obo:RO_0001025 rdf:resource="http://purl.obolibrary.org/obo/GAZ_00056820"/>
        <obo:IAO_0000115>A valley; on the Slovak side of the Western Tatras.</obo:IAO_0000115>
        <oboInOwl:hasOBONamespace>GAZ</oboInOwl:hasOBONamespace>
        <oboInOwl:id>GAZ:00481212</oboInOwl:id>
        <rdfs:label>Rachkova dolina</rdfs:label>
    </owl:NamedIndividual>
    


    <!-- http://purl.obolibrary.org/obo/GAZ_00481213 -->

    <owl:NamedIndividual rdf:about="http://purl.obolibrary.org/obo/GAZ_00481213">
        <obo:RO_0001025 rdf:resource="http://purl.obolibrary.org/obo/GAZ_00056820"/>
        <obo:IAO_0000115>A valley; on the Slovak side of the Western Tatras.</obo:IAO_0000115>
        <oboInOwl:hasOBONamespace>GAZ</oboInOwl:hasOBONamespace>
        <oboInOwl:id>GAZ:00481213</oboInOwl:id>
        <rdfs:label>Uzka dolina</rdfs:label>
    </owl:NamedIndividual>
    


    <!-- http://purl.obolibrary.org/obo/GAZ_00481214 -->

    <owl:NamedIndividual rdf:about="http://purl.obolibrary.org/obo/GAZ_00481214">
        <obo:RO_0001025 rdf:resource="http://purl.obolibrary.org/obo/GAZ_00056820"/>
        <obo:IAO_0000115>A valley; on the Slovak side of the Western Tatras.</obo:IAO_0000115>
        <oboInOwl:hasOBONamespace>GAZ</oboInOwl:hasOBONamespace>
        <oboInOwl:id>GAZ:00481214</oboInOwl:id>
        <rdfs:label>Kamenista dolina</rdfs:label>
    </owl:NamedIndividual>
    


    <!-- http://purl.obolibrary.org/obo/GAZ_00481215 -->

    <owl:NamedIndividual rdf:about="http://purl.obolibrary.org/obo/GAZ_00481215">
        <obo:RO_0001025 rdf:resource="http://purl.obolibrary.org/obo/GAZ_00481209"/>
        <obo:IAO_0000115>Five lakes.</obo:IAO_0000115>
        <oboInOwl:hasOBONamespace>GAZ</oboInOwl:hasOBONamespace>
        <oboInOwl:id>GAZ:00481215</oboInOwl:id>
        <rdfs:label>Gaborowe Stawki</rdfs:label>
    </owl:NamedIndividual>
    


    <!-- http://purl.obolibrary.org/obo/GAZ_00481216 -->

    <owl:NamedIndividual rdf:about="http://purl.obolibrary.org/obo/GAZ_00481216">
        <obo:RO_0001025 rdf:resource="http://purl.obolibrary.org/obo/GAZ_00007974"/>
        <obo:IAO_0000115>A valley.</obo:IAO_0000115>
        <oboInOwl:hasOBONamespace>GAZ</oboInOwl:hasOBONamespace>
        <oboInOwl:id>GAZ:00481216</oboInOwl:id>
        <rdfs:label>Slavkovska dolina</rdfs:label>
    </owl:NamedIndividual>
    


    <!-- http://purl.obolibrary.org/obo/GAZ_00481217 -->

    <owl:NamedIndividual rdf:about="http://purl.obolibrary.org/obo/GAZ_00481217">
        <obo:RO_0001025 rdf:resource="http://purl.obolibrary.org/obo/GAZ_00481216"/>
        <obo:IAO_0000115>A lake.</obo:IAO_0000115>
        <oboInOwl:hasOBONamespace>GAZ</oboInOwl:hasOBONamespace>
        <oboInOwl:id>GAZ:00481217</oboInOwl:id>
        <rdfs:label>Szontaghovo pleso</rdfs:label>
    </owl:NamedIndividual>
    


    <!-- http://purl.obolibrary.org/obo/GAZ_00481218 -->

    <owl:NamedIndividual rdf:about="http://purl.obolibrary.org/obo/GAZ_00481218">
        <obo:RO_0001025 rdf:resource="http://purl.obolibrary.org/obo/GAZ_00481216"/>
        <obo:IAO_0000115>A lake.</obo:IAO_0000115>
        <oboInOwl:hasOBONamespace>GAZ</oboInOwl:hasOBONamespace>
        <oboInOwl:id>GAZ:00481218</oboInOwl:id>
        <rdfs:label>Male Szontaghovo pliesko</rdfs:label>
    </owl:NamedIndividual>
    


    <!-- http://purl.obolibrary.org/obo/GAZ_00481219 -->

    <owl:NamedIndividual rdf:about="http://purl.obolibrary.org/obo/GAZ_00481219">
        <obo:RO_0001025 rdf:resource="http://purl.obolibrary.org/obo/GAZ_00481146"/>
        <obo:IAO_0000115>A lake.</obo:IAO_0000115>
        <oboInOwl:hasOBONamespace>GAZ</oboInOwl:hasOBONamespace>
        <oboInOwl:id>GAZ:00481219</oboInOwl:id>
        <rdfs:label>Horne Kvetnicove plieska</rdfs:label>
    </owl:NamedIndividual>
    


    <!-- http://purl.obolibrary.org/obo/GAZ_00481220 -->

    <owl:NamedIndividual rdf:about="http://purl.obolibrary.org/obo/GAZ_00481220">
        <obo:RO_0001025 rdf:resource="http://purl.obolibrary.org/obo/GAZ_00481211"/>
        <obo:IAO_0000115>A lake.</obo:IAO_0000115>
        <oboInOwl:hasOBONamespace>GAZ</oboInOwl:hasOBONamespace>
        <oboInOwl:id>GAZ:00481220</oboInOwl:id>
        <rdfs:label>Jamnicke plesa</rdfs:label>
    </owl:NamedIndividual>
    


    <!-- http://purl.obolibrary.org/obo/GAZ_00481221 -->

    <owl:NamedIndividual rdf:about="http://purl.obolibrary.org/obo/GAZ_00481221">
        <obo:RO_0001025 rdf:resource="http://purl.obolibrary.org/obo/GAZ_00007974"/>
        <obo:IAO_0000115>A valley.</obo:IAO_0000115>
        <oboInOwl:hasOBONamespace>GAZ</oboInOwl:hasOBONamespace>
        <oboInOwl:id>GAZ:00481221</oboInOwl:id>
        <rdfs:label>Vazecka dolina</rdfs:label>
    </owl:NamedIndividual>
    


    <!-- http://purl.obolibrary.org/obo/GAZ_00481222 -->

    <owl:NamedIndividual rdf:about="http://purl.obolibrary.org/obo/GAZ_00481222">
        <obo:RO_0001025 rdf:resource="http://purl.obolibrary.org/obo/GAZ_00481221"/>
        <obo:IAO_0000115>A lake.</obo:IAO_0000115>
        <oboInOwl:hasOBONamespace>GAZ</oboInOwl:hasOBONamespace>
        <oboInOwl:id>GAZ:00481222</oboInOwl:id>
        <rdfs:label>Jamske pleso</rdfs:label>
    </owl:NamedIndividual>
    


    <!-- http://purl.obolibrary.org/obo/GAZ_00481223 -->

    <owl:NamedIndividual rdf:about="http://purl.obolibrary.org/obo/GAZ_00481223">
        <obo:RO_0001025 rdf:resource="http://purl.obolibrary.org/obo/GAZ_00007974"/>
        <obo:IAO_0000115>A valley.</obo:IAO_0000115>
        <oboInOwl:hasOBONamespace>GAZ</oboInOwl:hasOBONamespace>
        <oboInOwl:id>GAZ:00481223</oboInOwl:id>
        <rdfs:label>Kachacia dolina</rdfs:label>
    </owl:NamedIndividual>
    


    <!-- http://purl.obolibrary.org/obo/GAZ_00481224 -->

    <owl:NamedIndividual rdf:about="http://purl.obolibrary.org/obo/GAZ_00481224">
        <obo:RO_0001025 rdf:resource="http://purl.obolibrary.org/obo/GAZ_00481223"/>
        <obo:IAO_0000115>A lake.</obo:IAO_0000115>
        <oboInOwl:hasOBONamespace>GAZ</oboInOwl:hasOBONamespace>
        <oboInOwl:id>GAZ:00481224</oboInOwl:id>
        <rdfs:label>Jelenie pliesko</rdfs:label>
    </owl:NamedIndividual>
    


    <!-- http://purl.obolibrary.org/obo/GAZ_00481226 -->

    <owl:NamedIndividual rdf:about="http://purl.obolibrary.org/obo/GAZ_00481226">
        <obo:IAO_0000115>A lake.</obo:IAO_0000115>
        <oboInOwl:hasOBONamespace>GAZ</oboInOwl:hasOBONamespace>
        <oboInOwl:id>GAZ:00481226</oboInOwl:id>
        <rdfs:label>Kobylie pliesko</rdfs:label>
    </owl:NamedIndividual>
    


    <!-- http://purl.obolibrary.org/obo/GAZ_00481227 -->

    <owl:NamedIndividual rdf:about="http://purl.obolibrary.org/obo/GAZ_00481227">
        <obo:RO_0001025 rdf:resource="http://purl.obolibrary.org/obo/GAZ_00481146"/>
        <obo:IAO_0000115>A lake.</obo:IAO_0000115>
        <oboInOwl:hasOBONamespace>GAZ</oboInOwl:hasOBONamespace>
        <oboInOwl:id>GAZ:00481227</oboInOwl:id>
        <rdfs:label>Kvetnicove pleso</rdfs:label>
    </owl:NamedIndividual>
    


    <!-- http://purl.obolibrary.org/obo/GAZ_00481228 -->

    <owl:NamedIndividual rdf:about="http://purl.obolibrary.org/obo/GAZ_00481228">
        <obo:IAO_0000115>A lake.</obo:IAO_0000115>
        <oboInOwl:hasOBONamespace>GAZ</oboInOwl:hasOBONamespace>
        <oboInOwl:id>GAZ:00481228</oboInOwl:id>
        <rdfs:label>Kolove pleso</rdfs:label>
    </owl:NamedIndividual>
    


    <!-- http://purl.obolibrary.org/obo/GAZ_00481229 -->

    <owl:NamedIndividual rdf:about="http://purl.obolibrary.org/obo/GAZ_00481229">
        <obo:RO_0001025 rdf:resource="http://purl.obolibrary.org/obo/GAZ_00007974"/>
        <obo:IAO_0000115>A valley.</obo:IAO_0000115>
        <oboInOwl:hasOBONamespace>GAZ</oboInOwl:hasOBONamespace>
        <oboInOwl:id>GAZ:00481229</oboInOwl:id>
        <rdfs:label>Litvorova dolina</rdfs:label>
    </owl:NamedIndividual>
    


    <!-- http://purl.obolibrary.org/obo/GAZ_00481230 -->

    <owl:NamedIndividual rdf:about="http://purl.obolibrary.org/obo/GAZ_00481230">
        <obo:RO_0001025 rdf:resource="http://purl.obolibrary.org/obo/GAZ_00481229"/>
        <obo:IAO_0000115>A lake.</obo:IAO_0000115>
        <oboInOwl:hasOBONamespace>GAZ</oboInOwl:hasOBONamespace>
        <oboInOwl:id>GAZ:00481230</oboInOwl:id>
        <rdfs:label>Litvorove pleso</rdfs:label>
    </owl:NamedIndividual>
    


    <!-- http://purl.obolibrary.org/obo/GAZ_00481231 -->

    <owl:NamedIndividual rdf:about="http://purl.obolibrary.org/obo/GAZ_00481231">
        <oboInOwl:hasOBONamespace>GAZ</oboInOwl:hasOBONamespace>
        <oboInOwl:id>GAZ:00481231</oboInOwl:id>
        <rdfs:label>Modre pleso</rdfs:label>
    </owl:NamedIndividual>
    


    <!-- http://purl.obolibrary.org/obo/GAZ_00481232 -->

    <owl:NamedIndividual rdf:about="http://purl.obolibrary.org/obo/GAZ_00481232">
        <obo:RO_0001025 rdf:resource="http://purl.obolibrary.org/obo/GAZ_00481094"/>
        <obo:IAO_0000115>A lake.</obo:IAO_0000115>
        <oboInOwl:hasOBONamespace>GAZ</oboInOwl:hasOBONamespace>
        <oboInOwl:id>GAZ:00481232</oboInOwl:id>
        <rdfs:label>Male Batizovske pliesko</rdfs:label>
    </owl:NamedIndividual>
    


    <!-- http://purl.obolibrary.org/obo/GAZ_00481233 -->

    <owl:NamedIndividual rdf:about="http://purl.obolibrary.org/obo/GAZ_00481233">
        <obo:RO_0001025 rdf:resource="http://purl.obolibrary.org/obo/GAZ_00481150"/>
        <obo:IAO_0000115>A valley.</obo:IAO_0000115>
        <oboInOwl:hasOBONamespace>GAZ</oboInOwl:hasOBONamespace>
        <oboInOwl:id>GAZ:00481233</oboInOwl:id>
        <rdfs:label>Kachacia dolina</rdfs:label>
    </owl:NamedIndividual>
    


    <!-- http://purl.obolibrary.org/obo/GAZ_00481234 -->

    <owl:NamedIndividual rdf:about="http://purl.obolibrary.org/obo/GAZ_00481234">
        <obo:RO_0001025 rdf:resource="http://purl.obolibrary.org/obo/GAZ_00481233"/>
        <obo:IAO_0000115>A lake.</obo:IAO_0000115>
        <oboInOwl:hasOBONamespace>GAZ</oboInOwl:hasOBONamespace>
        <oboInOwl:id>GAZ:00481234</oboInOwl:id>
        <rdfs:label>Kachacie pliesko</rdfs:label>
    </owl:NamedIndividual>
    


    <!-- http://purl.obolibrary.org/obo/GAZ_00481235 -->

    <owl:NamedIndividual rdf:about="http://purl.obolibrary.org/obo/GAZ_00481235">
        <obo:RO_0001025 rdf:resource="http://purl.obolibrary.org/obo/GAZ_00481102"/>
        <obo:IAO_0000115>A lake.</obo:IAO_0000115>
        <oboInOwl:hasOBONamespace>GAZ</oboInOwl:hasOBONamespace>
        <oboInOwl:id>GAZ:00481235</oboInOwl:id>
        <rdfs:label>Male Kozie pleso</rdfs:label>
    </owl:NamedIndividual>
    


    <!-- http://purl.obolibrary.org/obo/GAZ_00481237 -->

    <owl:NamedIndividual rdf:about="http://purl.obolibrary.org/obo/GAZ_00481237">
        <obo:IAO_0000115>A lake.</obo:IAO_0000115>
        <oboInOwl:hasOBONamespace>GAZ</oboInOwl:hasOBONamespace>
        <oboInOwl:id>GAZ:00481237</oboInOwl:id>
        <rdfs:label>Drachie pleso</rdfs:label>
    </owl:NamedIndividual>
    


    <!-- http://purl.obolibrary.org/obo/GAZ_00481238 -->

    <owl:NamedIndividual rdf:about="http://purl.obolibrary.org/obo/GAZ_00481238">
        <obo:IAO_0000115>A lake.</obo:IAO_0000115>
        <oboInOwl:hasOBONamespace>GAZ</oboInOwl:hasOBONamespace>
        <oboInOwl:id>GAZ:00481238</oboInOwl:id>
        <rdfs:label>Male Drachie pleso</rdfs:label>
    </owl:NamedIndividual>
    


    <!-- http://purl.obolibrary.org/obo/GAZ_00481239 -->

    <owl:NamedIndividual rdf:about="http://purl.obolibrary.org/obo/GAZ_00481239">
        <obo:IAO_0000115>A lake.</obo:IAO_0000115>
        <oboInOwl:hasOBONamespace>GAZ</oboInOwl:hasOBONamespace>
        <oboInOwl:id>GAZ:00481239</oboInOwl:id>
        <rdfs:label>Drachie oka</rdfs:label>
    </owl:NamedIndividual>
    


    <!-- http://purl.obolibrary.org/obo/GAZ_00481240 -->

    <owl:NamedIndividual rdf:about="http://purl.obolibrary.org/obo/GAZ_00481240">
        <obo:IAO_0000115>A lake.</obo:IAO_0000115>
        <oboInOwl:hasOBONamespace>GAZ</oboInOwl:hasOBONamespace>
        <oboInOwl:id>GAZ:00481240</oboInOwl:id>
        <rdfs:label>Male Cierne pleso</rdfs:label>
    </owl:NamedIndividual>
    


    <!-- http://purl.obolibrary.org/obo/GAZ_00481241 -->

    <owl:NamedIndividual rdf:about="http://purl.obolibrary.org/obo/GAZ_00481241">
        <obo:RO_0001025 rdf:resource="http://purl.obolibrary.org/obo/GAZ_00481221"/>
        <obo:IAO_0000115>A lake.</obo:IAO_0000115>
        <oboInOwl:hasOBONamespace>GAZ</oboInOwl:hasOBONamespace>
        <oboInOwl:id>GAZ:00481241</oboInOwl:id>
        <rdfs:label>Male Vazecke pliesko</rdfs:label>
    </owl:NamedIndividual>
    


    <!-- http://purl.obolibrary.org/obo/GAZ_00481242 -->

    <owl:NamedIndividual rdf:about="http://purl.obolibrary.org/obo/GAZ_00481242">
        <obo:IAO_0000115>A lake.</obo:IAO_0000115>
        <oboInOwl:hasOBONamespace>GAZ</oboInOwl:hasOBONamespace>
        <oboInOwl:id>GAZ:00481242</oboInOwl:id>
        <rdfs:label>Male Terianske pleso</rdfs:label>
    </owl:NamedIndividual>
    


    <!-- http://purl.obolibrary.org/obo/GAZ_00481243 -->

    <owl:NamedIndividual rdf:about="http://purl.obolibrary.org/obo/GAZ_00481243">
        <obo:IAO_0000115>A lake.</obo:IAO_0000115>
        <oboInOwl:hasOBONamespace>GAZ</oboInOwl:hasOBONamespace>
        <oboInOwl:id>GAZ:00481243</oboInOwl:id>
        <rdfs:label>Maly Zmarzly Stawek</rdfs:label>
    </owl:NamedIndividual>
    


    <!-- http://purl.obolibrary.org/obo/GAZ_00481245 -->

    <owl:NamedIndividual rdf:about="http://purl.obolibrary.org/obo/GAZ_00481245">
        <obo:IAO_0000115>A lake.</obo:IAO_0000115>
        <oboInOwl:hasOBONamespace>GAZ</oboInOwl:hasOBONamespace>
        <oboInOwl:id>GAZ:00481245</oboInOwl:id>
        <rdfs:label>Male Zabie Javorove pleso</rdfs:label>
    </owl:NamedIndividual>
    


    <!-- http://purl.obolibrary.org/obo/GAZ_00481246 -->

    <owl:NamedIndividual rdf:about="http://purl.obolibrary.org/obo/GAZ_00481246">
        <obo:RO_0001025 rdf:resource="http://purl.obolibrary.org/obo/GAZ_00481178"/>
        <obo:IAO_0000115>A valley.</obo:IAO_0000115>
        <oboInOwl:hasOBONamespace>GAZ</oboInOwl:hasOBONamespace>
        <oboInOwl:id>GAZ:00481246</oboInOwl:id>
        <rdfs:label>Zabia dolina mengusovska</rdfs:label>
    </owl:NamedIndividual>
    


    <!-- http://purl.obolibrary.org/obo/GAZ_00481247 -->

    <owl:NamedIndividual rdf:about="http://purl.obolibrary.org/obo/GAZ_00481247">
        <obo:RO_0001025 rdf:resource="http://purl.obolibrary.org/obo/GAZ_00481246"/>
        <obo:IAO_0000115>A lake in the High Tatras.</obo:IAO_0000115>
        <oboInOwl:hasOBONamespace>GAZ</oboInOwl:hasOBONamespace>
        <oboInOwl:id>GAZ:00481247</oboInOwl:id>
        <rdfs:label>Vel&apos;ke Zabie pleso mengusovske</rdfs:label>
    </owl:NamedIndividual>
    


    <!-- http://purl.obolibrary.org/obo/GAZ_00481248 -->

    <owl:NamedIndividual rdf:about="http://purl.obolibrary.org/obo/GAZ_00481248">
        <obo:RO_0001025 rdf:resource="http://purl.obolibrary.org/obo/GAZ_00481246"/>
        <obo:IAO_0000115>A lake.</obo:IAO_0000115>
        <oboInOwl:hasOBONamespace>GAZ</oboInOwl:hasOBONamespace>
        <oboInOwl:id>GAZ:00481248</oboInOwl:id>
        <rdfs:label>Male Zabie pleso mengusovske</rdfs:label>
    </owl:NamedIndividual>
    


    <!-- http://purl.obolibrary.org/obo/GAZ_00481249 -->

    <owl:NamedIndividual rdf:about="http://purl.obolibrary.org/obo/GAZ_00481249">
        <obo:RO_0001025 rdf:resource="http://purl.obolibrary.org/obo/GAZ_00481246"/>
        <obo:IAO_0000115>A lake.</obo:IAO_0000115>
        <oboInOwl:hasOBONamespace>GAZ</oboInOwl:hasOBONamespace>
        <oboInOwl:id>GAZ:00481249</oboInOwl:id>
        <rdfs:label>Vysne Zabie pleso mengusovske</rdfs:label>
    </owl:NamedIndividual>
    


    <!-- http://purl.obolibrary.org/obo/GAZ_00481250 -->

    <owl:NamedIndividual rdf:about="http://purl.obolibrary.org/obo/GAZ_00481250">
        <obo:IAO_0000115>A lake.</obo:IAO_0000115>
        <oboInOwl:hasOBONamespace>GAZ</oboInOwl:hasOBONamespace>
        <oboInOwl:id>GAZ:00481250</oboInOwl:id>
        <rdfs:label>Nizne Temnosmrechinske pleso</rdfs:label>
    </owl:NamedIndividual>
    


    <!-- http://purl.obolibrary.org/obo/GAZ_00481251 -->

    <owl:NamedIndividual rdf:about="http://purl.obolibrary.org/obo/GAZ_00481251">
        <obo:IAO_0000115>A lake.</obo:IAO_0000115>
        <oboInOwl:hasOBONamespace>GAZ</oboInOwl:hasOBONamespace>
        <oboInOwl:id>GAZ:00481251</oboInOwl:id>
        <rdfs:label>Nizne Sesterske pleso</rdfs:label>
    </owl:NamedIndividual>
    


    <!-- http://purl.obolibrary.org/obo/GAZ_00481252 -->

    <owl:NamedIndividual rdf:about="http://purl.obolibrary.org/obo/GAZ_00481252">
        <obo:IAO_0000115>A lake.</obo:IAO_0000115>
        <oboInOwl:hasOBONamespace>GAZ</oboInOwl:hasOBONamespace>
        <oboInOwl:id>GAZ:00481252</oboInOwl:id>
        <rdfs:label>Vysne Sesterske pleso</rdfs:label>
    </owl:NamedIndividual>
    


    <!-- http://purl.obolibrary.org/obo/GAZ_00481253 -->

    <owl:NamedIndividual rdf:about="http://purl.obolibrary.org/obo/GAZ_00481253">
        <obo:RO_0001025 rdf:resource="http://purl.obolibrary.org/obo/GAZ_00481140"/>
        <obo:IAO_0000115>A lake.</obo:IAO_0000115>
        <oboInOwl:hasOBONamespace>GAZ</oboInOwl:hasOBONamespace>
        <oboInOwl:id>GAZ:00481253</oboInOwl:id>
        <rdfs:label>Nizne Sive pleso</rdfs:label>
    </owl:NamedIndividual>
    


    <!-- http://purl.obolibrary.org/obo/GAZ_00481254 -->

    <owl:NamedIndividual rdf:about="http://purl.obolibrary.org/obo/GAZ_00481254">
        <obo:RO_0001025 rdf:resource="http://purl.obolibrary.org/obo/GAZ_00481140"/>
        <obo:IAO_0000115>A lake.</obo:IAO_0000115>
        <oboInOwl:hasOBONamespace>GAZ</oboInOwl:hasOBONamespace>
        <oboInOwl:id>GAZ:00481254</oboInOwl:id>
        <rdfs:label>Prostredne Sive pleso</rdfs:label>
    </owl:NamedIndividual>
    


    <!-- http://purl.obolibrary.org/obo/GAZ_00481255 -->

    <owl:NamedIndividual rdf:about="http://purl.obolibrary.org/obo/GAZ_00481255">
        <obo:RO_0001025 rdf:resource="http://purl.obolibrary.org/obo/GAZ_00481140"/>
        <obo:IAO_0000115>A lake.</obo:IAO_0000115>
        <oboInOwl:hasOBONamespace>GAZ</oboInOwl:hasOBONamespace>
        <oboInOwl:id>GAZ:00481255</oboInOwl:id>
        <rdfs:label>Vysne Sive pleso</rdfs:label>
    </owl:NamedIndividual>
    


    <!-- http://purl.obolibrary.org/obo/GAZ_00481256 -->

    <owl:NamedIndividual rdf:about="http://purl.obolibrary.org/obo/GAZ_00481256">
        <obo:RO_0001025 rdf:resource="http://purl.obolibrary.org/obo/GAZ_00481211"/>
        <obo:IAO_0000115>A lake.</obo:IAO_0000115>
        <oboInOwl:hasOBONamespace>GAZ</oboInOwl:hasOBONamespace>
        <oboInOwl:id>GAZ:00481256</oboInOwl:id>
        <rdfs:label>Nizne Jamnicke pleso</rdfs:label>
    </owl:NamedIndividual>
    


    <!-- http://purl.obolibrary.org/obo/GAZ_00481257 -->

    <owl:NamedIndividual rdf:about="http://purl.obolibrary.org/obo/GAZ_00481257">
        <obo:RO_0001025 rdf:resource="http://purl.obolibrary.org/obo/GAZ_00481183"/>
        <obo:IAO_0000115>A lake.</obo:IAO_0000115>
        <oboInOwl:hasOBONamespace>GAZ</oboInOwl:hasOBONamespace>
        <oboInOwl:id>GAZ:00481257</oboInOwl:id>
        <rdfs:label>Nizne Furkotske pliesko</rdfs:label>
    </owl:NamedIndividual>
    


    <!-- http://purl.obolibrary.org/obo/GAZ_00481258 -->

    <owl:NamedIndividual rdf:about="http://purl.obolibrary.org/obo/GAZ_00481258">
        <obo:IAO_0000115>A lake.</obo:IAO_0000115>
        <oboInOwl:hasOBONamespace>GAZ</oboInOwl:hasOBONamespace>
        <oboInOwl:id>GAZ:00481258</oboInOwl:id>
        <rdfs:label>Nizne Studene pleso</rdfs:label>
    </owl:NamedIndividual>
    


    <!-- http://purl.obolibrary.org/obo/GAZ_00481259 -->

    <owl:NamedIndividual rdf:about="http://purl.obolibrary.org/obo/GAZ_00481259">
        <obo:RO_0001025 rdf:resource="http://purl.obolibrary.org/obo/GAZ_00007974"/>
        <obo:IAO_0000115>Lakes.</obo:IAO_0000115>
        <oboInOwl:hasOBONamespace>GAZ</oboInOwl:hasOBONamespace>
        <oboInOwl:id>GAZ:00481259</oboInOwl:id>
        <rdfs:label>Smrekovicke plieska</rdfs:label>
    </owl:NamedIndividual>
    


    <!-- http://purl.obolibrary.org/obo/GAZ_00481260 -->

    <owl:NamedIndividual rdf:about="http://purl.obolibrary.org/obo/GAZ_00481260">
        <obo:RO_0001025 rdf:resource="http://purl.obolibrary.org/obo/GAZ_00481259"/>
        <obo:IAO_0000115>A lake.</obo:IAO_0000115>
        <oboInOwl:hasOBONamespace>GAZ</oboInOwl:hasOBONamespace>
        <oboInOwl:id>GAZ:00481260</oboInOwl:id>
        <rdfs:label>Nizne Smrekovicke pliesko</rdfs:label>
    </owl:NamedIndividual>
    


    <!-- http://purl.obolibrary.org/obo/GAZ_00481261 -->

    <owl:NamedIndividual rdf:about="http://purl.obolibrary.org/obo/GAZ_00481261">
        <obo:RO_0001025 rdf:resource="http://purl.obolibrary.org/obo/GAZ_00481259"/>
        <obo:IAO_0000115>A lake.</obo:IAO_0000115>
        <oboInOwl:hasOBONamespace>GAZ</oboInOwl:hasOBONamespace>
        <oboInOwl:id>GAZ:00481261</oboInOwl:id>
        <rdfs:label>Vysne Smrekovicke pliesko</rdfs:label>
    </owl:NamedIndividual>
    


    <!-- http://purl.obolibrary.org/obo/GAZ_00481262 -->

    <owl:NamedIndividual rdf:about="http://purl.obolibrary.org/obo/GAZ_00481262">
        <obo:RO_0001025 rdf:resource="http://purl.obolibrary.org/obo/GAZ_00007974"/>
        <obo:IAO_0000115>Lakes.</obo:IAO_0000115>
        <oboInOwl:hasOBONamespace>GAZ</oboInOwl:hasOBONamespace>
        <oboInOwl:id>GAZ:00481262</oboInOwl:id>
        <rdfs:label>Rakytovske plieska</rdfs:label>
    </owl:NamedIndividual>
    


    <!-- http://purl.obolibrary.org/obo/GAZ_00481263 -->

    <owl:NamedIndividual rdf:about="http://purl.obolibrary.org/obo/GAZ_00481263">
        <obo:RO_0001025 rdf:resource="http://purl.obolibrary.org/obo/GAZ_00481262"/>
        <obo:IAO_0000115>A lake.</obo:IAO_0000115>
        <oboInOwl:hasOBONamespace>GAZ</oboInOwl:hasOBONamespace>
        <oboInOwl:id>GAZ:00481263</oboInOwl:id>
        <rdfs:label>Nizne Rakytovske pliesko</rdfs:label>
    </owl:NamedIndividual>
    


    <!-- http://purl.obolibrary.org/obo/GAZ_00481264 -->

    <owl:NamedIndividual rdf:about="http://purl.obolibrary.org/obo/GAZ_00481264">
        <obo:RO_0001025 rdf:resource="http://purl.obolibrary.org/obo/GAZ_00481262"/>
        <obo:IAO_0000115>A lake.</obo:IAO_0000115>
        <oboInOwl:hasOBONamespace>GAZ</oboInOwl:hasOBONamespace>
        <oboInOwl:id>GAZ:00481264</oboInOwl:id>
        <rdfs:label>Vysne Rakytovske pliesko</rdfs:label>
    </owl:NamedIndividual>
    


    <!-- http://purl.obolibrary.org/obo/GAZ_00481265 -->

    <owl:NamedIndividual rdf:about="http://purl.obolibrary.org/obo/GAZ_00481265">
        <obo:IAO_0000115>A lake.</obo:IAO_0000115>
        <oboInOwl:hasOBONamespace>GAZ</oboInOwl:hasOBONamespace>
        <oboInOwl:id>GAZ:00481265</oboInOwl:id>
        <rdfs:label>Stvrte Rohachske pleso</rdfs:label>
    </owl:NamedIndividual>
    


    <!-- http://purl.obolibrary.org/obo/GAZ_00481266 -->

    <owl:NamedIndividual rdf:about="http://purl.obolibrary.org/obo/GAZ_00481266">
        <obo:IAO_0000115>A lake.</obo:IAO_0000115>
        <oboInOwl:hasOBONamespace>GAZ</oboInOwl:hasOBONamespace>
        <oboInOwl:id>GAZ:00481266</oboInOwl:id>
        <rdfs:label>Druhe Rohachske pleso</rdfs:label>
    </owl:NamedIndividual>
    


    <!-- http://purl.obolibrary.org/obo/GAZ_00481267 -->

    <owl:NamedIndividual rdf:about="http://purl.obolibrary.org/obo/GAZ_00481267">
        <obo:IAO_0000115>A lake.</obo:IAO_0000115>
        <oboInOwl:hasOBONamespace>GAZ</oboInOwl:hasOBONamespace>
        <oboInOwl:id>GAZ:00481267</oboInOwl:id>
        <rdfs:label>Tretie Rohachske pleso</rdfs:label>
    </owl:NamedIndividual>
    


    <!-- http://purl.obolibrary.org/obo/GAZ_00481268 -->

    <owl:NamedIndividual rdf:about="http://purl.obolibrary.org/obo/GAZ_00481268">
        <obo:IAO_0000115>A lake.</obo:IAO_0000115>
        <oboInOwl:hasOBONamespace>GAZ</oboInOwl:hasOBONamespace>
        <oboInOwl:id>GAZ:00481268</oboInOwl:id>
        <rdfs:label>Wielki Staw Rohacki</rdfs:label>
    </owl:NamedIndividual>
    


    <!-- http://purl.obolibrary.org/obo/GAZ_00481269 -->

    <owl:NamedIndividual rdf:about="http://purl.obolibrary.org/obo/GAZ_00481269">
        <obo:IAO_0000115>A lake.</obo:IAO_0000115>
        <oboInOwl:hasOBONamespace>GAZ</oboInOwl:hasOBONamespace>
        <oboInOwl:id>GAZ:00481269</oboInOwl:id>
        <rdfs:label>Nizne Terianske pleso</rdfs:label>
    </owl:NamedIndividual>
    


    <!-- http://purl.obolibrary.org/obo/GAZ_00481270 -->

    <owl:NamedIndividual rdf:about="http://purl.obolibrary.org/obo/GAZ_00481270">
        <obo:RO_0001025 rdf:resource="http://purl.obolibrary.org/obo/GAZ_00007974"/>
        <obo:IAO_0000115>A valley.</obo:IAO_0000115>
        <oboInOwl:hasOBONamespace>GAZ</oboInOwl:hasOBONamespace>
        <oboInOwl:id>GAZ:00481270</oboInOwl:id>
        <rdfs:label>Zabia Bielovodska dolina</rdfs:label>
    </owl:NamedIndividual>
    


    <!-- http://purl.obolibrary.org/obo/GAZ_00481271 -->

    <owl:NamedIndividual rdf:about="http://purl.obolibrary.org/obo/GAZ_00481271">
        <obo:RO_0001025 rdf:resource="http://purl.obolibrary.org/obo/GAZ_00481270"/>
        <obo:IAO_0000115>A lake in the High Tatras.</obo:IAO_0000115>
        <oboInOwl:hasOBONamespace>GAZ</oboInOwl:hasOBONamespace>
        <oboInOwl:id>GAZ:00481271</oboInOwl:id>
        <rdfs:label>Nizne Zabie pleso Bialchanske</rdfs:label>
    </owl:NamedIndividual>
    


    <!-- http://purl.obolibrary.org/obo/GAZ_00481272 -->

    <owl:NamedIndividual rdf:about="http://purl.obolibrary.org/obo/GAZ_00481272">
        <obo:IAO_0000115>A lake.</obo:IAO_0000115>
        <oboInOwl:hasOBONamespace>GAZ</oboInOwl:hasOBONamespace>
        <oboInOwl:id>GAZ:00481272</oboInOwl:id>
        <rdfs:label>Nizne Spisske pleso</rdfs:label>
    </owl:NamedIndividual>
    


    <!-- http://purl.obolibrary.org/obo/GAZ_00481273 -->

    <owl:NamedIndividual rdf:about="http://purl.obolibrary.org/obo/GAZ_00481273">
        <obo:IAO_0000115>A lake.</obo:IAO_0000115>
        <oboInOwl:hasOBONamespace>GAZ</oboInOwl:hasOBONamespace>
        <oboInOwl:id>GAZ:00481273</oboInOwl:id>
        <rdfs:label>Prostredne Spisske pleso</rdfs:label>
    </owl:NamedIndividual>
    


    <!-- http://purl.obolibrary.org/obo/GAZ_00481274 -->

    <owl:NamedIndividual rdf:about="http://purl.obolibrary.org/obo/GAZ_00481274">
        <obo:IAO_0000115>A lake.</obo:IAO_0000115>
        <oboInOwl:hasOBONamespace>GAZ</oboInOwl:hasOBONamespace>
        <oboInOwl:id>GAZ:00481274</oboInOwl:id>
        <rdfs:label>Vysne Spisske pleso</rdfs:label>
    </owl:NamedIndividual>
    


    <!-- http://purl.obolibrary.org/obo/GAZ_00481275 -->

    <owl:NamedIndividual rdf:about="http://purl.obolibrary.org/obo/GAZ_00481275">
        <obo:IAO_0000115>A lake.</obo:IAO_0000115>
        <oboInOwl:hasOBONamespace>GAZ</oboInOwl:hasOBONamespace>
        <oboInOwl:id>GAZ:00481275</oboInOwl:id>
        <rdfs:label>Popradske pleso</rdfs:label>
    </owl:NamedIndividual>
    


    <!-- http://purl.obolibrary.org/obo/GAZ_00481276 -->

    <owl:NamedIndividual rdf:about="http://purl.obolibrary.org/obo/GAZ_00481276">
        <obo:RO_0001025 rdf:resource="http://purl.obolibrary.org/obo/GAZ_00481212"/>
        <obo:IAO_0000115>A lake.</obo:IAO_0000115>
        <oboInOwl:hasOBONamespace>GAZ</oboInOwl:hasOBONamespace>
        <oboInOwl:id>GAZ:00481276</oboInOwl:id>
        <rdfs:label>Nizne Rachkovo pleso</rdfs:label>
    </owl:NamedIndividual>
    


    <!-- http://purl.obolibrary.org/obo/GAZ_00481277 -->

    <owl:NamedIndividual rdf:about="http://purl.obolibrary.org/obo/GAZ_00481277">
        <obo:IAO_0000115>A lake.</obo:IAO_0000115>
        <oboInOwl:hasOBONamespace>GAZ</oboInOwl:hasOBONamespace>
        <oboInOwl:id>GAZ:00481277</oboInOwl:id>
        <rdfs:label>Puste oko</rdfs:label>
    </owl:NamedIndividual>
    


    <!-- http://purl.obolibrary.org/obo/GAZ_00481278 -->

    <owl:NamedIndividual rdf:about="http://purl.obolibrary.org/obo/GAZ_00481278">
        <obo:IAO_0000115>A lake.</obo:IAO_0000115>
        <oboInOwl:hasOBONamespace>GAZ</oboInOwl:hasOBONamespace>
        <oboInOwl:id>GAZ:00481278</oboInOwl:id>
        <rdfs:label>Puste pleso</rdfs:label>
    </owl:NamedIndividual>
    


    <!-- http://purl.obolibrary.org/obo/GAZ_00481280 -->

    <owl:NamedIndividual rdf:about="http://purl.obolibrary.org/obo/GAZ_00481280">
        <obo:IAO_0000115>A lake.</obo:IAO_0000115>
        <oboInOwl:hasOBONamespace>GAZ</oboInOwl:hasOBONamespace>
        <oboInOwl:id>GAZ:00481280</oboInOwl:id>
        <rdfs:label>Plachlive pliesko</rdfs:label>
    </owl:NamedIndividual>
    


    <!-- http://purl.obolibrary.org/obo/GAZ_00481281 -->

    <owl:NamedIndividual rdf:about="http://purl.obolibrary.org/obo/GAZ_00481281">
        <obo:RO_0001025 rdf:resource="http://purl.obolibrary.org/obo/GAZ_00056820"/>
    </owl:NamedIndividual>
    


    <!-- http://purl.obolibrary.org/obo/GAZ_00481283 -->

    <owl:NamedIndividual rdf:about="http://purl.obolibrary.org/obo/GAZ_00481283">
        <obo:RO_0001025 rdf:resource="http://purl.obolibrary.org/obo/GAZ_00007974"/>
        <obo:IAO_0000115>A valley.</obo:IAO_0000115>
        <oboInOwl:hasOBONamespace>GAZ</oboInOwl:hasOBONamespace>
        <oboInOwl:id>GAZ:00481283</oboInOwl:id>
        <rdfs:label>Rumanova dolinka</rdfs:label>
    </owl:NamedIndividual>
    


    <!-- http://purl.obolibrary.org/obo/GAZ_00481284 -->

    <owl:NamedIndividual rdf:about="http://purl.obolibrary.org/obo/GAZ_00481284">
        <obo:RO_0001025 rdf:resource="http://purl.obolibrary.org/obo/GAZ_00481283"/>
        <obo:IAO_0000115>A lake.</obo:IAO_0000115>
        <oboInOwl:hasOBONamespace>GAZ</oboInOwl:hasOBONamespace>
        <oboInOwl:id>GAZ:00481284</oboInOwl:id>
        <rdfs:label>Nizne Rumanovo pliesko</rdfs:label>
    </owl:NamedIndividual>
    


    <!-- http://purl.obolibrary.org/obo/GAZ_00481285 -->

    <owl:NamedIndividual rdf:about="http://purl.obolibrary.org/obo/GAZ_00481285">
        <obo:RO_0001025 rdf:resource="http://purl.obolibrary.org/obo/GAZ_00481283"/>
        <obo:IAO_0000115>A lake.</obo:IAO_0000115>
        <oboInOwl:hasOBONamespace>GAZ</oboInOwl:hasOBONamespace>
        <oboInOwl:id>GAZ:00481285</oboInOwl:id>
        <rdfs:label>Rumanovo pleso</rdfs:label>
    </owl:NamedIndividual>
    


    <!-- http://purl.obolibrary.org/obo/GAZ_00481286 -->

    <owl:NamedIndividual rdf:about="http://purl.obolibrary.org/obo/GAZ_00481286">
        <obo:RO_0001025 rdf:resource="http://purl.obolibrary.org/obo/GAZ_00481283"/>
        <obo:IAO_0000115>A lake.</obo:IAO_0000115>
        <oboInOwl:hasOBONamespace>GAZ</oboInOwl:hasOBONamespace>
        <oboInOwl:id>GAZ:00481286</oboInOwl:id>
        <rdfs:label>Vysne Rumanovo pliesko</rdfs:label>
    </owl:NamedIndividual>
    


    <!-- http://purl.obolibrary.org/obo/GAZ_00481287 -->

    <owl:NamedIndividual rdf:about="http://purl.obolibrary.org/obo/GAZ_00481287">
        <obo:RO_0001025 rdf:resource="http://purl.obolibrary.org/obo/GAZ_00481221"/>
        <obo:IAO_0000115>A lake.</obo:IAO_0000115>
        <oboInOwl:hasOBONamespace>GAZ</oboInOwl:hasOBONamespace>
        <oboInOwl:id>GAZ:00481287</oboInOwl:id>
        <rdfs:label>Skryte pliesko</rdfs:label>
    </owl:NamedIndividual>
    


    <!-- http://purl.obolibrary.org/obo/GAZ_00481288 -->

    <owl:NamedIndividual rdf:about="http://purl.obolibrary.org/obo/GAZ_00481288">
        <obo:RO_0001025 rdf:resource="http://purl.obolibrary.org/obo/GAZ_00481121"/>
        <obo:IAO_0000115>A lake.</obo:IAO_0000115>
        <oboInOwl:hasOBONamespace>GAZ</oboInOwl:hasOBONamespace>
        <oboInOwl:id>GAZ:00481288</oboInOwl:id>
        <rdfs:label>Sobkowe Oko</rdfs:label>
    </owl:NamedIndividual>
    


    <!-- http://purl.obolibrary.org/obo/GAZ_00481289 -->

    <owl:NamedIndividual rdf:about="http://purl.obolibrary.org/obo/GAZ_00481289">
        <obo:RO_0001025 rdf:resource="http://purl.obolibrary.org/obo/GAZ_00481183"/>
        <obo:IAO_0000115>A lake.</obo:IAO_0000115>
        <oboInOwl:hasOBONamespace>GAZ</oboInOwl:hasOBONamespace>
        <oboInOwl:id>GAZ:00481289</oboInOwl:id>
        <rdfs:label>Soliskove oko</rdfs:label>
    </owl:NamedIndividual>
    


    <!-- http://purl.obolibrary.org/obo/GAZ_00481290 -->

    <owl:NamedIndividual rdf:about="http://purl.obolibrary.org/obo/GAZ_00481290">
        <obo:IAO_0000115>A lake.</obo:IAO_0000115>
        <oboInOwl:hasOBONamespace>GAZ</oboInOwl:hasOBONamespace>
        <oboInOwl:id>GAZ:00481290</oboInOwl:id>
        <rdfs:label>Zbojnicke oko</rdfs:label>
    </owl:NamedIndividual>
    


    <!-- http://purl.obolibrary.org/obo/GAZ_00481291 -->

    <owl:NamedIndividual rdf:about="http://purl.obolibrary.org/obo/GAZ_00481291">
        <obo:IAO_0000115>A lake.</obo:IAO_0000115>
        <oboInOwl:hasOBONamespace>GAZ</oboInOwl:hasOBONamespace>
        <oboInOwl:id>GAZ:00481291</oboInOwl:id>
        <rdfs:label>Vysne Zbojnicke pleso</rdfs:label>
    </owl:NamedIndividual>
    


    <!-- http://purl.obolibrary.org/obo/GAZ_00481292 -->

    <owl:NamedIndividual rdf:about="http://purl.obolibrary.org/obo/GAZ_00481292">
        <obo:IAO_0000115>A lake.</obo:IAO_0000115>
        <oboInOwl:hasOBONamespace>GAZ</oboInOwl:hasOBONamespace>
        <oboInOwl:id>GAZ:00481292</oboInOwl:id>
        <rdfs:label>Vysne Studene pleso</rdfs:label>
    </owl:NamedIndividual>
    


    <!-- http://purl.obolibrary.org/obo/GAZ_00481293 -->

    <owl:NamedIndividual rdf:about="http://purl.obolibrary.org/obo/GAZ_00481293">
        <obo:RO_0001025 rdf:resource="http://purl.obolibrary.org/obo/GAZ_00481102"/>
        <obo:IAO_0000115>A lake.</obo:IAO_0000115>
        <oboInOwl:hasOBONamespace>GAZ</oboInOwl:hasOBONamespace>
        <oboInOwl:id>GAZ:00481293</oboInOwl:id>
        <rdfs:label>Pleso nad Skokom</rdfs:label>
    </owl:NamedIndividual>
    


    <!-- http://purl.obolibrary.org/obo/GAZ_00481294 -->

    <owl:NamedIndividual rdf:about="http://purl.obolibrary.org/obo/GAZ_00481294">
        <obo:RO_0001025 rdf:resource="http://purl.obolibrary.org/obo/GAZ_00481094"/>
        <obo:IAO_0000115>A lake.</obo:IAO_0000115>
        <oboInOwl:hasOBONamespace>GAZ</oboInOwl:hasOBONamespace>
        <oboInOwl:id>GAZ:00481294</oboInOwl:id>
        <rdfs:label>Pliesko pod Kostolikom</rdfs:label>
    </owl:NamedIndividual>
    


    <!-- http://purl.obolibrary.org/obo/GAZ_00481295 -->

    <owl:NamedIndividual rdf:about="http://purl.obolibrary.org/obo/GAZ_00481295">
        <obo:RO_0001025 rdf:resource="http://purl.obolibrary.org/obo/GAZ_00481131"/>
        <obo:IAO_0000115>Lakes.</obo:IAO_0000115>
        <oboInOwl:hasOBONamespace>GAZ</oboInOwl:hasOBONamespace>
        <oboInOwl:id>GAZ:00481295</oboInOwl:id>
        <rdfs:label>Pleso pod Zverovkou</rdfs:label>
    </owl:NamedIndividual>
    


    <!-- http://purl.obolibrary.org/obo/GAZ_00481296 -->

    <owl:NamedIndividual rdf:about="http://purl.obolibrary.org/obo/GAZ_00481296">
        <obo:RO_0001025 rdf:resource="http://purl.obolibrary.org/obo/GAZ_00481210"/>
        <obo:IAO_0000115>Lakes.</obo:IAO_0000115>
        <oboInOwl:hasOBONamespace>GAZ</oboInOwl:hasOBONamespace>
        <oboInOwl:id>GAZ:00481296</oboInOwl:id>
        <rdfs:label>Pliesko pod Ziarskom sedlom</rdfs:label>
    </owl:NamedIndividual>
    


    <!-- http://purl.obolibrary.org/obo/GAZ_00481297 -->

    <owl:NamedIndividual rdf:about="http://purl.obolibrary.org/obo/GAZ_00481297">
        <obo:RO_0001025 rdf:resource="http://purl.obolibrary.org/obo/GAZ_00481210"/>
        <obo:IAO_0000115>A lake.</obo:IAO_0000115>
        <oboInOwl:hasOBONamespace>GAZ</oboInOwl:hasOBONamespace>
        <oboInOwl:id>GAZ:00481297</oboInOwl:id>
        <rdfs:label>Ziarske sedlo</rdfs:label>
    </owl:NamedIndividual>
    


    <!-- http://purl.obolibrary.org/obo/GAZ_00481298 -->

    <owl:NamedIndividual rdf:about="http://purl.obolibrary.org/obo/GAZ_00481298">
        <obo:IAO_0000115>Lakes.</obo:IAO_0000115>
        <oboInOwl:hasOBONamespace>GAZ</oboInOwl:hasOBONamespace>
        <oboInOwl:id>GAZ:00481298</oboInOwl:id>
        <rdfs:label>Satanie plieska</rdfs:label>
    </owl:NamedIndividual>
    


    <!-- http://purl.obolibrary.org/obo/GAZ_00481299 -->

    <owl:NamedIndividual rdf:about="http://purl.obolibrary.org/obo/GAZ_00481299">
        <obo:RO_0001025 rdf:resource="http://purl.obolibrary.org/obo/GAZ_00481216"/>
        <obo:IAO_0000115>Lakes.</obo:IAO_0000115>
        <oboInOwl:hasOBONamespace>GAZ</oboInOwl:hasOBONamespace>
        <oboInOwl:id>GAZ:00481299</oboInOwl:id>
        <rdfs:label>Slavkovske pliesko</rdfs:label>
    </owl:NamedIndividual>
    


    <!-- http://purl.obolibrary.org/obo/GAZ_00481300 -->

    <owl:NamedIndividual rdf:about="http://purl.obolibrary.org/obo/GAZ_00481300">
        <obo:RO_0001025 rdf:resource="http://purl.obolibrary.org/obo/GAZ_00481216"/>
        <obo:IAO_0000115>Lakes.</obo:IAO_0000115>
        <oboInOwl:hasOBONamespace>GAZ</oboInOwl:hasOBONamespace>
        <oboInOwl:id>GAZ:00481300</oboInOwl:id>
        <rdfs:label>Slavkovske plieska</rdfs:label>
    </owl:NamedIndividual>
    


    <!-- http://purl.obolibrary.org/obo/GAZ_00481301 -->

    <owl:NamedIndividual rdf:about="http://purl.obolibrary.org/obo/GAZ_00481301">
        <obo:IAO_0000115>A lake.</obo:IAO_0000115>
        <oboInOwl:hasOBONamespace>GAZ</oboInOwl:hasOBONamespace>
        <oboInOwl:id>GAZ:00481301</oboInOwl:id>
        <rdfs:label>Vysne Terianske pleso</rdfs:label>
    </owl:NamedIndividual>
    


    <!-- http://purl.obolibrary.org/obo/GAZ_00481303 -->

    <owl:NamedIndividual rdf:about="http://purl.obolibrary.org/obo/GAZ_00481303">
        <obo:IAO_0000115>A lake.</obo:IAO_0000115>
        <oboInOwl:hasOBONamespace>GAZ</oboInOwl:hasOBONamespace>
        <oboInOwl:id>GAZ:00481303</oboInOwl:id>
        <rdfs:label>Male Tomanovske pleso</rdfs:label>
    </owl:NamedIndividual>
    


    <!-- http://purl.obolibrary.org/obo/GAZ_00481304 -->

    <owl:NamedIndividual rdf:about="http://purl.obolibrary.org/obo/GAZ_00481304">
        <obo:IAO_0000115>A lake.</obo:IAO_0000115>
        <oboInOwl:hasOBONamespace>GAZ</oboInOwl:hasOBONamespace>
        <oboInOwl:id>GAZ:00481304</oboInOwl:id>
        <rdfs:label>Vysne Tomanovske pleso</rdfs:label>
    </owl:NamedIndividual>
    


    <!-- http://purl.obolibrary.org/obo/GAZ_00481305 -->

    <owl:NamedIndividual rdf:about="http://purl.obolibrary.org/obo/GAZ_00481305">
        <obo:IAO_0000115>A lake.</obo:IAO_0000115>
        <oboInOwl:hasOBONamespace>GAZ</oboInOwl:hasOBONamespace>
        <oboInOwl:id>GAZ:00481305</oboInOwl:id>
        <rdfs:label>Nizne Tomanovske pleso</rdfs:label>
    </owl:NamedIndividual>
    


    <!-- http://purl.obolibrary.org/obo/GAZ_00481307 -->

    <owl:NamedIndividual rdf:about="http://purl.obolibrary.org/obo/GAZ_00481307">
        <obo:RO_0001025 rdf:resource="http://purl.obolibrary.org/obo/GAZ_00481146"/>
        <obo:IAO_0000115>A lake.</obo:IAO_0000115>
        <oboInOwl:hasOBONamespace>GAZ</oboInOwl:hasOBONamespace>
        <oboInOwl:id>GAZ:00481307</oboInOwl:id>
        <rdfs:label>Velicke pleso</rdfs:label>
    </owl:NamedIndividual>
    


    <!-- http://purl.obolibrary.org/obo/GAZ_00481308 -->

    <owl:NamedIndividual rdf:about="http://purl.obolibrary.org/obo/GAZ_00481308">
        <obo:RO_0001025 rdf:resource="http://purl.obolibrary.org/obo/GAZ_00481146"/>
        <obo:IAO_0000115>A lake.</obo:IAO_0000115>
        <oboInOwl:hasOBONamespace>GAZ</oboInOwl:hasOBONamespace>
        <oboInOwl:id>GAZ:00481308</oboInOwl:id>
        <rdfs:label>Vysne Velicke plieska</rdfs:label>
    </owl:NamedIndividual>
    


    <!-- http://purl.obolibrary.org/obo/GAZ_00481309 -->

    <owl:NamedIndividual rdf:about="http://purl.obolibrary.org/obo/GAZ_00481309">
        <obo:IAO_0000115>A lake.</obo:IAO_0000115>
        <oboInOwl:hasOBONamespace>GAZ</oboInOwl:hasOBONamespace>
        <oboInOwl:id>GAZ:00481309</oboInOwl:id>
        <rdfs:label>Velke Biele pleso</rdfs:label>
    </owl:NamedIndividual>
    


    <!-- http://purl.obolibrary.org/obo/GAZ_00481310 -->

    <owl:NamedIndividual rdf:about="http://purl.obolibrary.org/obo/GAZ_00481310">
        <obo:IAO_0000115>A lake.</obo:IAO_0000115>
        <oboInOwl:hasOBONamespace>GAZ</oboInOwl:hasOBONamespace>
        <oboInOwl:id>GAZ:00481310</oboInOwl:id>
        <rdfs:label>Vysne Temnosmrechinske pleso</rdfs:label>
    </owl:NamedIndividual>
    


    <!-- http://purl.obolibrary.org/obo/GAZ_00481311 -->

    <owl:NamedIndividual rdf:about="http://purl.obolibrary.org/obo/GAZ_00481311">
        <obo:RO_0001025 rdf:resource="http://purl.obolibrary.org/obo/GAZ_00481211"/>
        <obo:IAO_0000115>A lake.</obo:IAO_0000115>
        <oboInOwl:hasOBONamespace>GAZ</oboInOwl:hasOBONamespace>
        <oboInOwl:id>GAZ:00481311</oboInOwl:id>
        <rdfs:label>Vysne Jamnicke pleso</rdfs:label>
    </owl:NamedIndividual>
    


    <!-- http://purl.obolibrary.org/obo/GAZ_00481312 -->

    <owl:NamedIndividual rdf:about="http://purl.obolibrary.org/obo/GAZ_00481312">
        <obo:RO_0001025 rdf:resource="http://purl.obolibrary.org/obo/GAZ_00481183"/>
        <obo:IAO_0000115>A lake.</obo:IAO_0000115>
        <oboInOwl:hasOBONamespace>GAZ</oboInOwl:hasOBONamespace>
        <oboInOwl:id>GAZ:00481312</oboInOwl:id>
        <rdfs:label>Vysne Furkotske pliesko</rdfs:label>
    </owl:NamedIndividual>
    


    <!-- http://purl.obolibrary.org/obo/GAZ_00481313 -->

    <owl:NamedIndividual rdf:about="http://purl.obolibrary.org/obo/GAZ_00481313">
        <obo:RO_0001025 rdf:resource="http://purl.obolibrary.org/obo/GAZ_00481183"/>
        <obo:IAO_0000115>A lake.</obo:IAO_0000115>
        <oboInOwl:hasOBONamespace>GAZ</oboInOwl:hasOBONamespace>
        <oboInOwl:id>GAZ:00481313</oboInOwl:id>
        <rdfs:label>Vysne Wahlenbergovo pleso</rdfs:label>
    </owl:NamedIndividual>
    


    <!-- http://purl.obolibrary.org/obo/GAZ_00481314 -->

    <owl:NamedIndividual rdf:about="http://purl.obolibrary.org/obo/GAZ_00481314">
        <obo:RO_0001025 rdf:resource="http://purl.obolibrary.org/obo/GAZ_00481270"/>
        <obo:IAO_0000115>A lake in the High Tatras.</obo:IAO_0000115>
        <oboInOwl:hasOBONamespace>GAZ</oboInOwl:hasOBONamespace>
        <oboInOwl:id>GAZ:00481314</oboInOwl:id>
        <rdfs:label>Vysne Zabie pleso Bialchanske</rdfs:label>
    </owl:NamedIndividual>
    


    <!-- http://purl.obolibrary.org/obo/GAZ_00481316 -->

    <owl:NamedIndividual rdf:about="http://purl.obolibrary.org/obo/GAZ_00481316">
        <obo:IAO_0000115>Lakes.</obo:IAO_0000115>
        <oboInOwl:hasOBONamespace>GAZ</oboInOwl:hasOBONamespace>
        <oboInOwl:id>GAZ:00481316</oboInOwl:id>
        <rdfs:label>Stratene pliesko</rdfs:label>
    </owl:NamedIndividual>
    


    <!-- http://purl.obolibrary.org/obo/GAZ_00481318 -->

    <owl:NamedIndividual rdf:about="http://purl.obolibrary.org/obo/GAZ_00481318">
        <obo:IAO_0000115>A lake.</obo:IAO_0000115>
        <oboInOwl:hasOBONamespace>GAZ</oboInOwl:hasOBONamespace>
        <oboInOwl:id>GAZ:00481318</oboInOwl:id>
        <rdfs:label>Zelene Javorove pleso)</rdfs:label>
    </owl:NamedIndividual>
    


    <!-- http://purl.obolibrary.org/obo/GAZ_00481319 -->

    <owl:NamedIndividual rdf:about="http://purl.obolibrary.org/obo/GAZ_00481319">
        <obo:RO_0001025 rdf:resource="http://purl.obolibrary.org/obo/GAZ_00481223"/>
        <obo:IAO_0000115>A lake.</obo:IAO_0000115>
        <oboInOwl:hasOBONamespace>GAZ</oboInOwl:hasOBONamespace>
        <oboInOwl:id>GAZ:00481319</oboInOwl:id>
        <rdfs:label>Zelene Kachacie pleso</rdfs:label>
    </owl:NamedIndividual>
    


    <!-- http://purl.obolibrary.org/obo/GAZ_00481320 -->

    <owl:NamedIndividual rdf:about="http://purl.obolibrary.org/obo/GAZ_00481320">
        <obo:RO_0001025 rdf:resource="http://purl.obolibrary.org/obo/GAZ_00481160"/>
        <obo:IAO_0000115>A lake.</obo:IAO_0000115>
        <oboInOwl:hasOBONamespace>GAZ</oboInOwl:hasOBONamespace>
        <oboInOwl:id>GAZ:00481320</oboInOwl:id>
        <rdfs:label>Zelene pleso</rdfs:label>
    </owl:NamedIndividual>
    


    <!-- http://purl.obolibrary.org/obo/GAZ_00481321 -->

    <owl:NamedIndividual rdf:about="http://purl.obolibrary.org/obo/GAZ_00481321">
        <obo:RO_0001025 rdf:resource="http://purl.obolibrary.org/obo/GAZ_00481221"/>
        <obo:IAO_0000115>A lake.</obo:IAO_0000115>
        <oboInOwl:hasOBONamespace>GAZ</oboInOwl:hasOBONamespace>
        <oboInOwl:id>GAZ:00481321</oboInOwl:id>
        <rdfs:label>Zelene pleso Krivanske</rdfs:label>
    </owl:NamedIndividual>
    


    <!-- http://purl.obolibrary.org/obo/GAZ_00481322 -->

    <owl:NamedIndividual rdf:about="http://purl.obolibrary.org/obo/GAZ_00481322">
        <obo:IAO_0000115>A lake.</obo:IAO_0000115>
        <oboInOwl:hasOBONamespace>GAZ</oboInOwl:hasOBONamespace>
        <oboInOwl:id>GAZ:00481322</oboInOwl:id>
        <rdfs:label>Zelene pliesko</rdfs:label>
    </owl:NamedIndividual>
    


    <!-- http://purl.obolibrary.org/obo/GAZ_00481323 -->

    <owl:NamedIndividual rdf:about="http://purl.obolibrary.org/obo/GAZ_00481323">
        <obo:RO_0001025 rdf:resource="http://purl.obolibrary.org/obo/GAZ_00007974"/>
        <obo:IAO_0000115>A valley.</obo:IAO_0000115>
        <oboInOwl:hasOBONamespace>GAZ</oboInOwl:hasOBONamespace>
        <oboInOwl:id>GAZ:00481323</oboInOwl:id>
        <rdfs:label>Svistova dolina</rdfs:label>
    </owl:NamedIndividual>
    


    <!-- http://purl.obolibrary.org/obo/GAZ_00481324 -->

    <owl:NamedIndividual rdf:about="http://purl.obolibrary.org/obo/GAZ_00481324">
        <obo:IAO_0000115>A lake.</obo:IAO_0000115>
        <oboInOwl:hasOBONamespace>GAZ</oboInOwl:hasOBONamespace>
        <oboInOwl:id>GAZ:00481324</oboInOwl:id>
        <rdfs:label>Zamrznute pleso</rdfs:label>
    </owl:NamedIndividual>
    


    <!-- http://purl.obolibrary.org/obo/GAZ_00481325 -->

    <owl:NamedIndividual rdf:about="http://purl.obolibrary.org/obo/GAZ_00481325">
        <obo:IAO_0000115>A lake.</obo:IAO_0000115>
        <oboInOwl:hasOBONamespace>GAZ</oboInOwl:hasOBONamespace>
        <oboInOwl:id>GAZ:00481325</oboInOwl:id>
        <rdfs:label>Zamrznute oka</rdfs:label>
    </owl:NamedIndividual>
    


    <!-- http://purl.obolibrary.org/obo/GAZ_00481326 -->

    <owl:NamedIndividual rdf:about="http://purl.obolibrary.org/obo/GAZ_00481326">
        <obo:RO_0001025 rdf:resource="http://purl.obolibrary.org/obo/GAZ_00481115"/>
        <obo:IAO_0000115>A lake in the High Tatras.</obo:IAO_0000115>
        <oboInOwl:hasOBONamespace>GAZ</oboInOwl:hasOBONamespace>
        <oboInOwl:id>GAZ:00481326</oboInOwl:id>
        <rdfs:label>Zmrzle pleso</rdfs:label>
    </owl:NamedIndividual>
    


    <!-- http://purl.obolibrary.org/obo/GAZ_00481327 -->

    <owl:NamedIndividual rdf:about="http://purl.obolibrary.org/obo/GAZ_00481327">
        <obo:RO_0001025 rdf:resource="http://purl.obolibrary.org/obo/GAZ_00007974"/>
        <obo:IAO_0000115>A valley.</obo:IAO_0000115>
        <oboInOwl:hasOBONamespace>GAZ</oboInOwl:hasOBONamespace>
        <oboInOwl:id>GAZ:00481327</oboInOwl:id>
        <rdfs:label>Skalnata dolina</rdfs:label>
    </owl:NamedIndividual>
    


    <!-- http://purl.obolibrary.org/obo/GAZ_00481328 -->

    <owl:NamedIndividual rdf:about="http://purl.obolibrary.org/obo/GAZ_00481328">
        <obo:RO_0001025 rdf:resource="http://purl.obolibrary.org/obo/GAZ_00481327"/>
        <obo:IAO_0000115>A lake.</obo:IAO_0000115>
        <oboInOwl:hasOBONamespace>GAZ</oboInOwl:hasOBONamespace>
        <oboInOwl:id>GAZ:00481328</oboInOwl:id>
        <rdfs:label>Skalnate pleso</rdfs:label>
    </owl:NamedIndividual>
    


    <!-- http://purl.obolibrary.org/obo/GAZ_00481329 -->

    <owl:NamedIndividual rdf:about="http://purl.obolibrary.org/obo/GAZ_00481329">
        <obo:RO_0001025 rdf:resource="http://purl.obolibrary.org/obo/GAZ_00481327"/>
        <obo:IAO_0000115>A lake.</obo:IAO_0000115>
        <oboInOwl:hasOBONamespace>GAZ</oboInOwl:hasOBONamespace>
        <oboInOwl:id>GAZ:00481329</oboInOwl:id>
        <rdfs:label>Skalnate oko</rdfs:label>
    </owl:NamedIndividual>
    


    <!-- http://purl.obolibrary.org/obo/GAZ_00481330 -->

    <owl:NamedIndividual rdf:about="http://purl.obolibrary.org/obo/GAZ_00481330">
        <obo:RO_0001025 rdf:resource="http://purl.obolibrary.org/obo/GAZ_00481323"/>
        <obo:IAO_0000115>Lakes.</obo:IAO_0000115>
        <oboInOwl:hasOBONamespace>GAZ</oboInOwl:hasOBONamespace>
        <oboInOwl:id>GAZ:00481330</oboInOwl:id>
        <rdfs:label>Hrube plesa</rdfs:label>
    </owl:NamedIndividual>
    


    <!-- http://purl.obolibrary.org/obo/GAZ_00481331 -->

    <owl:NamedIndividual rdf:about="http://purl.obolibrary.org/obo/GAZ_00481331">
        <obo:IAO_0000115>A lake.</obo:IAO_0000115>
        <oboInOwl:hasOBONamespace>GAZ</oboInOwl:hasOBONamespace>
        <oboInOwl:id>GAZ:00481331</oboInOwl:id>
        <rdfs:label>Zabie pleso Javorove</rdfs:label>
    </owl:NamedIndividual>
    


    <!-- http://purl.obolibrary.org/obo/GAZ_00481332 -->

    <owl:NamedIndividual rdf:about="http://purl.obolibrary.org/obo/GAZ_00481332">
        <obo:IAO_0000115>A lake.</obo:IAO_0000115>
        <oboInOwl:hasOBONamespace>GAZ</oboInOwl:hasOBONamespace>
        <oboInOwl:id>GAZ:00481332</oboInOwl:id>
        <rdfs:label>Stawek na Kopkach</rdfs:label>
    </owl:NamedIndividual>
    


    <!-- http://purl.obolibrary.org/obo/GAZ_00481333 -->

    <owl:NamedIndividual rdf:about="http://purl.obolibrary.org/obo/GAZ_00481333">
        <obo:IAO_0000115>A lake.</obo:IAO_0000115>
        <oboInOwl:hasOBONamespace>GAZ</oboInOwl:hasOBONamespace>
        <oboInOwl:id>GAZ:00481333</oboInOwl:id>
        <rdfs:label>Male Morskie Oko</rdfs:label>
    </owl:NamedIndividual>
    


    <!-- http://purl.obolibrary.org/obo/GAZ_00481334 -->

    <owl:NamedIndividual rdf:about="http://purl.obolibrary.org/obo/GAZ_00481334">
        <obo:IAO_0000115>A lake.</obo:IAO_0000115>
        <oboInOwl:hasOBONamespace>GAZ</oboInOwl:hasOBONamespace>
        <oboInOwl:id>GAZ:00481334</oboInOwl:id>
        <rdfs:label>Zabie Oko</rdfs:label>
    </owl:NamedIndividual>
    


    <!-- http://purl.obolibrary.org/obo/GAZ_00481335 -->

    <owl:NamedIndividual rdf:about="http://purl.obolibrary.org/obo/GAZ_00481335">
        <obo:IAO_0000115>A lake.</obo:IAO_0000115>
        <oboInOwl:hasOBONamespace>GAZ</oboInOwl:hasOBONamespace>
        <oboInOwl:id>GAZ:00481335</oboInOwl:id>
        <rdfs:label>Male Zabie Oko</rdfs:label>
    </owl:NamedIndividual>
    


    <!-- http://purl.obolibrary.org/obo/GAZ_00481668 -->

    <owl:NamedIndividual rdf:about="http://purl.obolibrary.org/obo/GAZ_00481668">
        <obo:RO_0001025 rdf:resource="http://purl.obolibrary.org/obo/GAZ_00061932"/>
        <obo:IAO_0000115>A protected area.</obo:IAO_0000115>
        <oboInOwl:hasOBONamespace>GAZ</oboInOwl:hasOBONamespace>
        <oboInOwl:id>GAZ:00481668</oboInOwl:id>
        <rdfs:label>Rezerwat przyrody Kornuty</rdfs:label>
    </owl:NamedIndividual>
    


    <!-- http://purl.obolibrary.org/obo/GAZ_00482221 -->

    <owl:NamedIndividual rdf:about="http://purl.obolibrary.org/obo/GAZ_00482221">
        <obo:IAO_0000115>A reservoir.</obo:IAO_0000115>
        <oboInOwl:hasOBONamespace>GAZ</oboInOwl:hasOBONamespace>
        <oboInOwl:id>GAZ:00482221</oboInOwl:id>
        <rdfs:label>Jezioro Czchowskie</rdfs:label>
    </owl:NamedIndividual>
    


    <!-- http://purl.obolibrary.org/obo/GAZ_00482222 -->

    <owl:NamedIndividual rdf:about="http://purl.obolibrary.org/obo/GAZ_00482222">
        <obo:IAO_0000115>A reservoir.</obo:IAO_0000115>
        <oboInOwl:hasOBONamespace>GAZ</oboInOwl:hasOBONamespace>
        <oboInOwl:id>GAZ:00482222</oboInOwl:id>
        <rdfs:label>Sromowce</rdfs:label>
    </owl:NamedIndividual>
    


    <!-- http://purl.obolibrary.org/obo/GAZ_00595723 -->

    <owl:NamedIndividual rdf:about="http://purl.obolibrary.org/obo/GAZ_00595723">
        <rdf:type rdf:resource="http://purl.obolibrary.org/obo/ENVO_00000423"/>
        <obo:IAO_0000115>A fluvial island.</obo:IAO_0000115>
        <oboInOwl:hasOBONamespace>GAZ</oboInOwl:hasOBONamespace>
        <oboInOwl:id>GAZ:00595723</oboInOwl:id>
        <rdfs:label>Muhleninsel</rdfs:label>
    </owl:NamedIndividual>
    


    <!-- http://purl.obolibrary.org/obo/GAZ_00595724 -->

    <owl:NamedIndividual rdf:about="http://purl.obolibrary.org/obo/GAZ_00595724">
        <rdf:type rdf:resource="http://purl.obolibrary.org/obo/ENVO_00000423"/>
        <obo:IAO_0000115>A fluvial island.</obo:IAO_0000115>
        <oboInOwl:hasOBONamespace>GAZ</oboInOwl:hasOBONamespace>
        <oboInOwl:id>GAZ:00595724</oboInOwl:id>
        <rdfs:label>Museumsinsel</rdfs:label>
    </owl:NamedIndividual>
    


    <!-- http://purl.obolibrary.org/obo/GAZ_00595725 -->

    <owl:NamedIndividual rdf:about="http://purl.obolibrary.org/obo/GAZ_00595725">
        <rdf:type rdf:resource="http://purl.obolibrary.org/obo/ENVO_00000423"/>
        <obo:IAO_0000115>A fluvial island.</obo:IAO_0000115>
        <oboInOwl:hasOBONamespace>GAZ</oboInOwl:hasOBONamespace>
        <oboInOwl:id>GAZ:00595725</oboInOwl:id>
        <rdfs:label>Praterinsel</rdfs:label>
    </owl:NamedIndividual>
    


    <!-- http://purl.obolibrary.org/obo/GAZ_00598025 -->

    <owl:NamedIndividual rdf:about="http://purl.obolibrary.org/obo/GAZ_00598025">
        <obo:IAO_0000115>A river.</obo:IAO_0000115>
        <oboInOwl:hasOBONamespace>GAZ</oboInOwl:hasOBONamespace>
        <oboInOwl:id>GAZ:00598025</oboInOwl:id>
        <rdfs:label>Schollach</rdfs:label>
    </owl:NamedIndividual>
    


    <!-- http://purl.obolibrary.org/obo/GAZ_00598026 -->

    <owl:NamedIndividual rdf:about="http://purl.obolibrary.org/obo/GAZ_00598026">
        <obo:IAO_0000115>A river.</obo:IAO_0000115>
        <oboInOwl:hasOBONamespace>GAZ</oboInOwl:hasOBONamespace>
        <oboInOwl:id>GAZ:00598026</oboInOwl:id>
        <rdfs:label>Bubenbachle</rdfs:label>
    </owl:NamedIndividual>
    


    <!-- http://purl.obolibrary.org/obo/GAZ_00601431 -->

    <owl:NamedIndividual rdf:about="http://purl.obolibrary.org/obo/GAZ_00601431">
        <obo:IAO_0000115>A sinkhole. An incipient underground stream capture in the Upper Danube Nature Park. Between Immendingen and Mohringen and also near Fridingen (Tuttlingen), the water of the Danube sinks into the riverbed in various places. The main sinkhole is next to a field named Bruhl between Immendingen and Mohringen. The sinking Danube water disappears into a karst water system and appears again in a horizontal limestone layer (the ki4 layer), approximately twelve kilometers away at Aachtopf. It then flows as Radolfzeller Aach into Lake Constance at Radolfzell.</obo:IAO_0000115>
        <oboInOwl:hasOBONamespace>GAZ</oboInOwl:hasOBONamespace>
        <oboInOwl:id>GAZ:00601431</oboInOwl:id>
        <rdfs:label>Donauversinkung</rdfs:label>
    </owl:NamedIndividual>
    


    <!-- http://purl.obolibrary.org/obo/GAZ_00604501 -->

    <owl:NamedIndividual rdf:about="http://purl.obolibrary.org/obo/GAZ_00604501">
        <obo:IAO_0000115>A reservoir.</obo:IAO_0000115>
        <oboInOwl:hasOBONamespace>GAZ</oboInOwl:hasOBONamespace>
        <oboInOwl:id>GAZ:00604501</oboInOwl:id>
        <rdfs:label>Stausee Tannheim</rdfs:label>
    </owl:NamedIndividual>
    


    <!-- http://purl.obolibrary.org/obo/GAZ_00604502 -->

    <owl:NamedIndividual rdf:about="http://purl.obolibrary.org/obo/GAZ_00604502">
        <obo:IAO_0000115>A reservoir.</obo:IAO_0000115>
        <oboInOwl:hasOBONamespace>GAZ</oboInOwl:hasOBONamespace>
        <oboInOwl:id>GAZ:00604502</oboInOwl:id>
        <rdfs:label>Stausee Dettingen</rdfs:label>
    </owl:NamedIndividual>
    


    <!-- http://purl.obolibrary.org/obo/GAZ_00606233 -->

    <owl:NamedIndividual rdf:about="http://purl.obolibrary.org/obo/GAZ_00606233">
        <obo:IAO_0000115>A river.</obo:IAO_0000115>
        <oboInOwl:hasOBONamespace>GAZ</oboInOwl:hasOBONamespace>
        <oboInOwl:id>GAZ:00606233</oboInOwl:id>
        <rdfs:label>Argelsbach</rdfs:label>
    </owl:NamedIndividual>
    


    <!-- http://purl.obolibrary.org/obo/GAZ_00606545 -->

    <owl:NamedIndividual rdf:about="http://purl.obolibrary.org/obo/GAZ_00606545">
        <obo:IAO_0000115>A dam.</obo:IAO_0000115>
        <oboInOwl:hasOBONamespace>GAZ</oboInOwl:hasOBONamespace>
        <oboInOwl:id>GAZ:00606545</oboInOwl:id>
        <rdfs:label>Brandbachtalsperre</rdfs:label>
    </owl:NamedIndividual>
    


    <!-- http://purl.obolibrary.org/obo/GAZ_00606557 -->

    <owl:NamedIndividual rdf:about="http://purl.obolibrary.org/obo/GAZ_00606557">
        <obo:IAO_0000115>A dam.</obo:IAO_0000115>
        <oboInOwl:hasOBONamespace>GAZ</oboInOwl:hasOBONamespace>
        <oboInOwl:id>GAZ:00606557</oboInOwl:id>
        <rdfs:label>Linachtalsperre</rdfs:label>
    </owl:NamedIndividual>
    


    <!-- http://purl.obolibrary.org/obo/GAZ_00606739 -->

    <owl:NamedIndividual rdf:about="http://purl.obolibrary.org/obo/GAZ_00606739">
        <obo:IAO_0000115>A lake.</obo:IAO_0000115>
        <oboInOwl:hasOBONamespace>GAZ</oboInOwl:hasOBONamespace>
        <oboInOwl:id>GAZ:00606739</oboInOwl:id>
        <rdfs:label>Tannschorrenweiher</rdfs:label>
    </owl:NamedIndividual>
    


    <!-- http://purl.obolibrary.org/obo/GAZ_00607104 -->

    <owl:NamedIndividual rdf:about="http://purl.obolibrary.org/obo/GAZ_00607104">
        <obo:IAO_0000115>A populated place. A district (Ortsteil).</obo:IAO_0000115>
        <oboInOwl:hasOBONamespace>GAZ</oboInOwl:hasOBONamespace>
        <oboInOwl:id>GAZ:00607104</oboInOwl:id>
        <rdfs:label>Gunzenhausen</rdfs:label>
    </owl:NamedIndividual>
    


    <!-- http://purl.obolibrary.org/obo/GAZ_00607332 -->

    <owl:NamedIndividual rdf:about="http://purl.obolibrary.org/obo/GAZ_00607332">
        <obo:RO_0001025 rdf:resource="http://purl.obolibrary.org/obo/GAZ_00061537"/>
        <obo:IAO_0000115>A dam on the Schwarzach.</obo:IAO_0000115>
        <oboInOwl:hasOBONamespace>GAZ</oboInOwl:hasOBONamespace>
        <oboInOwl:id>GAZ:00607332</oboInOwl:id>
        <rdfs:label>Talsperre Eixendorf</rdfs:label>
    </owl:NamedIndividual>
    


    <!-- http://purl.obolibrary.org/obo/GAZ_00607595 -->

    <owl:NamedIndividual rdf:about="http://purl.obolibrary.org/obo/GAZ_00607595">
        <obo:IAO_0000115>A lake; located on Staatsstrasse 2019 (Krumbach - Weissenhorn) between Deisenhausen and Ingstetten.</obo:IAO_0000115>
        <oboInOwl:hasOBONamespace>GAZ</oboInOwl:hasOBONamespace>
        <oboInOwl:id>GAZ:00607595</oboInOwl:id>
        <rdfs:label>Ingstetter Weiher</rdfs:label>
    </owl:NamedIndividual>
    


    <!-- http://purl.obolibrary.org/obo/GAZ_00607925 -->

    <owl:NamedIndividual rdf:about="http://purl.obolibrary.org/obo/GAZ_00607925">
        <obo:IAO_0000115>A dam.</obo:IAO_0000115>
        <oboInOwl:hasOBONamespace>GAZ</oboInOwl:hasOBONamespace>
        <oboInOwl:id>GAZ:00607925</oboInOwl:id>
        <rdfs:label>Lechstaustufe 2 - Prem</rdfs:label>
    </owl:NamedIndividual>
    


    <!-- http://purl.obolibrary.org/obo/GAZ_00607926 -->

    <owl:NamedIndividual rdf:about="http://purl.obolibrary.org/obo/GAZ_00607926">
        <obo:IAO_0000115>A dam.</obo:IAO_0000115>
        <oboInOwl:hasOBONamespace>GAZ</oboInOwl:hasOBONamespace>
        <oboInOwl:id>GAZ:00607926</oboInOwl:id>
        <rdfs:label>Lechstaustufe 22 - Unterbergen</rdfs:label>
    </owl:NamedIndividual>
    


    <!-- http://purl.obolibrary.org/obo/GAZ_00607927 -->

    <owl:NamedIndividual rdf:about="http://purl.obolibrary.org/obo/GAZ_00607927">
        <obo:IAO_0000115>A dam.</obo:IAO_0000115>
        <oboInOwl:hasOBONamespace>GAZ</oboInOwl:hasOBONamespace>
        <oboInOwl:id>GAZ:00607927</oboInOwl:id>
        <rdfs:label>Lechstaustufe 6 - Dornau</rdfs:label>
    </owl:NamedIndividual>
    


    <!-- http://purl.obolibrary.org/obo/GAZ_00607928 -->

    <owl:NamedIndividual rdf:about="http://purl.obolibrary.org/obo/GAZ_00607928">
        <obo:IAO_0000115>A dam; located between Landsberg am Lech and Augsburg.</obo:IAO_0000115>
        <oboInOwl:hasOBONamespace>GAZ</oboInOwl:hasOBONamespace>
        <oboInOwl:id>GAZ:00607928</oboInOwl:id>
        <rdfs:label>Lechstaustufe 23 - Merching</rdfs:label>
    </owl:NamedIndividual>
    


    <!-- http://purl.obolibrary.org/obo/GAZ_00609434 -->

    <owl:NamedIndividual rdf:about="http://purl.obolibrary.org/obo/GAZ_00609434">
        <obo:IAO_0000115>A lake.</obo:IAO_0000115>
        <oboInOwl:hasOBONamespace>GAZ</oboInOwl:hasOBONamespace>
        <oboInOwl:id>GAZ:00609434</oboInOwl:id>
        <rdfs:label>Rottachsee</rdfs:label>
    </owl:NamedIndividual>
    


    <!-- http://purl.obolibrary.org/obo/GAZ_00609567 -->

    <owl:NamedIndividual rdf:about="http://purl.obolibrary.org/obo/GAZ_00609567">
        <obo:IAO_0000115>A hydroelectric power station.</obo:IAO_0000115>
        <oboInOwl:hasOBONamespace>GAZ</oboInOwl:hasOBONamespace>
        <oboInOwl:id>GAZ:00609567</oboInOwl:id>
        <rdfs:label>Walchenseekraftwerk</rdfs:label>
    </owl:NamedIndividual>
    


    <!-- http://purl.obolibrary.org/obo/GAZ_00612221 -->

    <owl:NamedIndividual rdf:about="http://purl.obolibrary.org/obo/GAZ_00612221">
        <obo:IAO_0000115>A former canal. It linked the Danube River at Kelheim with the Main River at Bamberg, connecting the Danube basin with the Rhine basin.</obo:IAO_0000115>
        <oboInOwl:hasOBONamespace>GAZ</oboInOwl:hasOBONamespace>
        <oboInOwl:id>GAZ:00612221</oboInOwl:id>
        <rdfs:label>Ludwig-Donau-Main-Kanal</rdfs:label>
    </owl:NamedIndividual>
    


    <!-- http://purl.obolibrary.org/obo/GAZ_00612272 -->

    <owl:NamedIndividual rdf:about="http://purl.obolibrary.org/obo/GAZ_00612272">
        <obo:IAO_0000115>A lock.</obo:IAO_0000115>
        <oboInOwl:hasOBONamespace>GAZ</oboInOwl:hasOBONamespace>
        <oboInOwl:id>GAZ:00612272</oboInOwl:id>
        <rdfs:label>Schleuse Leerstetten</rdfs:label>
    </owl:NamedIndividual>
    


    <!-- http://purl.obolibrary.org/obo/GAZ_00612914 -->

    <owl:NamedIndividual rdf:about="http://purl.obolibrary.org/obo/GAZ_00612914">
        <obo:IAO_0000115>A river.</obo:IAO_0000115>
        <oboInOwl:hasOBONamespace>GAZ</oboInOwl:hasOBONamespace>
        <oboInOwl:id>GAZ:00612914</oboInOwl:id>
        <rdfs:label>Anifer Alterbach</rdfs:label>
    </owl:NamedIndividual>
    


    <!-- http://purl.obolibrary.org/obo/GAZ_00612959 -->

    <owl:NamedIndividual rdf:about="http://purl.obolibrary.org/obo/GAZ_00612959">
        <obo:IAO_0000115>A river.</obo:IAO_0000115>
        <oboInOwl:hasOBONamespace>GAZ</oboInOwl:hasOBONamespace>
        <oboInOwl:id>GAZ:00612959</oboInOwl:id>
        <rdfs:label>Kleine Isar</rdfs:label>
    </owl:NamedIndividual>
    


    <!-- http://purl.obolibrary.org/obo/GAZ_00612967 -->

    <owl:NamedIndividual rdf:about="http://purl.obolibrary.org/obo/GAZ_00612967">
        <obo:IAO_0000115>A river.</obo:IAO_0000115>
        <oboInOwl:hasOBONamespace>GAZ</oboInOwl:hasOBONamespace>
        <oboInOwl:id>GAZ:00612967</oboInOwl:id>
        <rdfs:label>Weissenbach</rdfs:label>
    </owl:NamedIndividual>
    


    <!-- http://purl.obolibrary.org/obo/GAZ_00612968 -->

    <owl:NamedIndividual rdf:about="http://purl.obolibrary.org/obo/GAZ_00612968">
        <obo:IAO_0000115>A river.</obo:IAO_0000115>
        <oboInOwl:hasOBONamespace>GAZ</oboInOwl:hasOBONamespace>
        <oboInOwl:id>GAZ:00612968</oboInOwl:id>
        <rdfs:label>Bayerbach</rdfs:label>
    </owl:NamedIndividual>
    


    <!-- http://purl.obolibrary.org/obo/GAZ_00612969 -->

    <owl:NamedIndividual rdf:about="http://purl.obolibrary.org/obo/GAZ_00612969">
        <obo:IAO_0000115>A river.</obo:IAO_0000115>
        <oboInOwl:hasOBONamespace>GAZ</oboInOwl:hasOBONamespace>
        <oboInOwl:id>GAZ:00612969</oboInOwl:id>
        <rdfs:label>Hengstbach</rdfs:label>
    </owl:NamedIndividual>
    


    <!-- http://purl.obolibrary.org/obo/GAZ_00612970 -->

    <owl:NamedIndividual rdf:about="http://purl.obolibrary.org/obo/GAZ_00612970">
        <obo:IAO_0000115>A river.</obo:IAO_0000115>
        <oboInOwl:hasOBONamespace>GAZ</oboInOwl:hasOBONamespace>
        <oboInOwl:id>GAZ:00612970</oboInOwl:id>
        <rdfs:label>Rehgraben</rdfs:label>
    </owl:NamedIndividual>
    


    <!-- http://purl.obolibrary.org/obo/GAZ_00612971 -->

    <owl:NamedIndividual rdf:about="http://purl.obolibrary.org/obo/GAZ_00612971">
        <obo:IAO_0000115>A river.</obo:IAO_0000115>
        <oboInOwl:hasOBONamespace>GAZ</oboInOwl:hasOBONamespace>
        <oboInOwl:id>GAZ:00612971</oboInOwl:id>
        <rdfs:label>Kohlgraben</rdfs:label>
    </owl:NamedIndividual>
    


    <!-- http://purl.obolibrary.org/obo/GAZ_00612972 -->

    <owl:NamedIndividual rdf:about="http://purl.obolibrary.org/obo/GAZ_00612972">
        <obo:IAO_0000115>A river.</obo:IAO_0000115>
        <oboInOwl:hasOBONamespace>GAZ</oboInOwl:hasOBONamespace>
        <oboInOwl:id>GAZ:00612972</oboInOwl:id>
        <rdfs:label>Riebgraben</rdfs:label>
    </owl:NamedIndividual>
    


    <!-- http://purl.obolibrary.org/obo/GAZ_00612973 -->

    <owl:NamedIndividual rdf:about="http://purl.obolibrary.org/obo/GAZ_00612973">
        <obo:IAO_0000115>A river.</obo:IAO_0000115>
        <oboInOwl:hasOBONamespace>GAZ</oboInOwl:hasOBONamespace>
        <oboInOwl:id>GAZ:00612973</oboInOwl:id>
        <rdfs:label>Trogellahnegraben</rdfs:label>
    </owl:NamedIndividual>
    


    <!-- http://purl.obolibrary.org/obo/GAZ_00612974 -->

    <owl:NamedIndividual rdf:about="http://purl.obolibrary.org/obo/GAZ_00612974">
        <obo:IAO_0000115>A river.</obo:IAO_0000115>
        <oboInOwl:hasOBONamespace>GAZ</oboInOwl:hasOBONamespace>
        <oboInOwl:id>GAZ:00612974</oboInOwl:id>
        <rdfs:label>Leimbach</rdfs:label>
    </owl:NamedIndividual>
    


    <!-- http://purl.obolibrary.org/obo/GAZ_00613056 -->

    <owl:NamedIndividual rdf:about="http://purl.obolibrary.org/obo/GAZ_00613056">
        <obo:IAO_0000115>A reservoir.</obo:IAO_0000115>
        <oboInOwl:hasOBONamespace>GAZ</oboInOwl:hasOBONamespace>
        <oboInOwl:id>GAZ:00613056</oboInOwl:id>
        <rdfs:label>Stausee Altheim</rdfs:label>
    </owl:NamedIndividual>
    


    <!-- http://purl.obolibrary.org/obo/GAZ_00613057 -->

    <owl:NamedIndividual rdf:about="http://purl.obolibrary.org/obo/GAZ_00613057">
        <obo:IAO_0000115>A reservoir.</obo:IAO_0000115>
        <oboInOwl:hasOBONamespace>GAZ</oboInOwl:hasOBONamespace>
        <oboInOwl:id>GAZ:00613057</oboInOwl:id>
        <rdfs:label>Stauweiher</rdfs:label>
    </owl:NamedIndividual>
    


    <!-- http://purl.obolibrary.org/obo/GAZ_00613058 -->

    <owl:NamedIndividual rdf:about="http://purl.obolibrary.org/obo/GAZ_00613058">
        <obo:IAO_0000115>A reservoir.</obo:IAO_0000115>
        <oboInOwl:hasOBONamespace>GAZ</oboInOwl:hasOBONamespace>
        <oboInOwl:id>GAZ:00613058</oboInOwl:id>
        <rdfs:label>Stausee Niederaichbach</rdfs:label>
    </owl:NamedIndividual>
    


    <!-- http://purl.obolibrary.org/obo/GAZ_00613061 -->

    <owl:NamedIndividual rdf:about="http://purl.obolibrary.org/obo/GAZ_00613061">
        <obo:IAO_0000115>A reservoir.</obo:IAO_0000115>
        <oboInOwl:hasOBONamespace>GAZ</oboInOwl:hasOBONamespace>
        <oboInOwl:id>GAZ:00613061</oboInOwl:id>
        <rdfs:label>Stausee Oberilzmuhle</rdfs:label>
    </owl:NamedIndividual>
    


    <!-- http://purl.obolibrary.org/obo/GAZ_00613294 -->

    <owl:NamedIndividual rdf:about="http://purl.obolibrary.org/obo/GAZ_00613294">
        <obo:IAO_0000115>A river.</obo:IAO_0000115>
        <oboInOwl:hasOBONamespace>GAZ</oboInOwl:hasOBONamespace>
        <oboInOwl:id>GAZ:00613294</oboInOwl:id>
        <rdfs:label>Goldbach</rdfs:label>
    </owl:NamedIndividual>
    


    <!-- http://purl.obolibrary.org/obo/GAZ_00613295 -->

    <owl:NamedIndividual rdf:about="http://purl.obolibrary.org/obo/GAZ_00613295">
        <obo:IAO_0000115>A river.</obo:IAO_0000115>
        <oboInOwl:hasOBONamespace>GAZ</oboInOwl:hasOBONamespace>
        <oboInOwl:id>GAZ:00613295</oboInOwl:id>
        <rdfs:label>Grunbach</rdfs:label>
    </owl:NamedIndividual>
    


    <!-- http://purl.obolibrary.org/obo/GAZ_00613296 -->

    <owl:NamedIndividual rdf:about="http://purl.obolibrary.org/obo/GAZ_00613296">
        <obo:IAO_0000115>A river.</obo:IAO_0000115>
        <oboInOwl:hasOBONamespace>GAZ</oboInOwl:hasOBONamespace>
        <oboInOwl:id>GAZ:00613296</oboInOwl:id>
        <rdfs:label>Feuerbach</rdfs:label>
    </owl:NamedIndividual>
    


    <!-- http://purl.obolibrary.org/obo/GAZ_00613297 -->

    <owl:NamedIndividual rdf:about="http://purl.obolibrary.org/obo/GAZ_00613297">
        <obo:IAO_0000115>A river.</obo:IAO_0000115>
        <oboInOwl:hasOBONamespace>GAZ</oboInOwl:hasOBONamespace>
        <oboInOwl:id>GAZ:00613297</oboInOwl:id>
        <rdfs:label>Stachelbach</rdfs:label>
    </owl:NamedIndividual>
    


    <!-- http://purl.obolibrary.org/obo/GAZ_00613298 -->

    <owl:NamedIndividual rdf:about="http://purl.obolibrary.org/obo/GAZ_00613298">
        <obo:IAO_0000115>A river.</obo:IAO_0000115>
        <oboInOwl:hasOBONamespace>GAZ</oboInOwl:hasOBONamespace>
        <oboInOwl:id>GAZ:00613298</oboInOwl:id>
        <rdfs:label>Wernhardsberger Graben</rdfs:label>
    </owl:NamedIndividual>
    


    <!-- http://purl.obolibrary.org/obo/GAZ_00613299 -->

    <owl:NamedIndividual rdf:about="http://purl.obolibrary.org/obo/GAZ_00613299">
        <obo:IAO_0000115>A river.</obo:IAO_0000115>
        <oboInOwl:hasOBONamespace>GAZ</oboInOwl:hasOBONamespace>
        <oboInOwl:id>GAZ:00613299</oboInOwl:id>
        <rdfs:label>Buchgraben</rdfs:label>
    </owl:NamedIndividual>
    


    <!-- http://purl.obolibrary.org/obo/GAZ_00613300 -->

    <owl:NamedIndividual rdf:about="http://purl.obolibrary.org/obo/GAZ_00613300">
        <obo:IAO_0000115>A river.</obo:IAO_0000115>
        <oboInOwl:hasOBONamespace>GAZ</oboInOwl:hasOBONamespace>
        <oboInOwl:id>GAZ:00613300</oboInOwl:id>
        <rdfs:label>Weizenbach</rdfs:label>
    </owl:NamedIndividual>
    


    <!-- http://purl.obolibrary.org/obo/GAZ_00613301 -->

    <owl:NamedIndividual rdf:about="http://purl.obolibrary.org/obo/GAZ_00613301">
        <obo:IAO_0000115>A river.</obo:IAO_0000115>
        <oboInOwl:hasOBONamespace>GAZ</oboInOwl:hasOBONamespace>
        <oboInOwl:id>GAZ:00613301</oboInOwl:id>
        <rdfs:label>Steinbach</rdfs:label>
    </owl:NamedIndividual>
    


    <!-- http://purl.obolibrary.org/obo/GAZ_00613302 -->

    <owl:NamedIndividual rdf:about="http://purl.obolibrary.org/obo/GAZ_00613302">
        <obo:IAO_0000115>A river.</obo:IAO_0000115>
        <oboInOwl:hasOBONamespace>GAZ</oboInOwl:hasOBONamespace>
        <oboInOwl:id>GAZ:00613302</oboInOwl:id>
        <rdfs:label>Schachener Graben</rdfs:label>
    </owl:NamedIndividual>
    


    <!-- http://purl.obolibrary.org/obo/GAZ_00613303 -->

    <owl:NamedIndividual rdf:about="http://purl.obolibrary.org/obo/GAZ_00613303">
        <obo:IAO_0000115>A river.</obo:IAO_0000115>
        <oboInOwl:hasOBONamespace>GAZ</oboInOwl:hasOBONamespace>
        <oboInOwl:id>GAZ:00613303</oboInOwl:id>
        <rdfs:label>Rimbach</rdfs:label>
    </owl:NamedIndividual>
    


    <!-- http://purl.obolibrary.org/obo/GAZ_00613304 -->

    <owl:NamedIndividual rdf:about="http://purl.obolibrary.org/obo/GAZ_00613304">
        <obo:IAO_0000115>A river.</obo:IAO_0000115>
        <oboInOwl:hasOBONamespace>GAZ</oboInOwl:hasOBONamespace>
        <oboInOwl:id>GAZ:00613304</oboInOwl:id>
        <rdfs:label>Ornaubach</rdfs:label>
    </owl:NamedIndividual>
    


    <!-- http://purl.obolibrary.org/obo/GAZ_00619830 -->

    <owl:NamedIndividual rdf:about="http://purl.obolibrary.org/obo/GAZ_00619830"/>
    


    <!-- http://purl.obolibrary.org/obo/GAZ_00619876 -->

    <owl:NamedIndividual rdf:about="http://purl.obolibrary.org/obo/GAZ_00619876">
        <obo:IAO_0000115>A hydroelectric power station.</obo:IAO_0000115>
        <oboInOwl:hasOBONamespace>GAZ</oboInOwl:hasOBONamespace>
        <oboInOwl:id>GAZ:00619876</oboInOwl:id>
        <rdfs:label>Isarwerk 1</rdfs:label>
    </owl:NamedIndividual>
    


    <!-- http://purl.obolibrary.org/obo/GAZ_00619897 -->

    <owl:NamedIndividual rdf:about="http://purl.obolibrary.org/obo/GAZ_00619897">
        <obo:RO_0001025 rdf:resource="http://purl.obolibrary.org/obo/GAZ_00619830"/>
        <obo:IAO_0000115>A hydroelectric power station.</obo:IAO_0000115>
        <oboInOwl:hasOBONamespace>GAZ</oboInOwl:hasOBONamespace>
        <oboInOwl:id>GAZ:00619897</oboInOwl:id>
        <rdfs:label>Isarwerk 2</rdfs:label>
    </owl:NamedIndividual>
    


    <!-- http://purl.obolibrary.org/obo/GAZ_00619898 -->

    <owl:NamedIndividual rdf:about="http://purl.obolibrary.org/obo/GAZ_00619898">
        <obo:RO_0001025 rdf:resource="http://purl.obolibrary.org/obo/GAZ_00619830"/>
        <oboInOwl:hasOBONamespace>GAZ</oboInOwl:hasOBONamespace>
        <oboInOwl:id>GAZ:00619898</oboInOwl:id>
        <rdfs:label>Isarwerk 3</rdfs:label>
    </owl:NamedIndividual>
    


    <!-- http://purl.obolibrary.org/obo/GAZ_00619923 -->

    <owl:NamedIndividual rdf:about="http://purl.obolibrary.org/obo/GAZ_00619923">
        <rdf:type rdf:resource="http://purl.obolibrary.org/obo/ENVO_00000423"/>
        <obo:IAO_0000115>A fluvial island.</obo:IAO_0000115>
        <oboInOwl:hasOBONamespace>GAZ</oboInOwl:hasOBONamespace>
        <oboInOwl:id>GAZ:00619923</oboInOwl:id>
        <rdfs:label>Feuerwerksinsel</rdfs:label>
    </owl:NamedIndividual>
    


    <!-- http://purl.obolibrary.org/obo/GAZ_00619924 -->

    <owl:NamedIndividual rdf:about="http://purl.obolibrary.org/obo/GAZ_00619924">
        <rdf:type rdf:resource="http://purl.obolibrary.org/obo/ENVO_00000423"/>
        <obo:IAO_0000115>A fluvial island.</obo:IAO_0000115>
        <oboInOwl:hasOBONamespace>GAZ</oboInOwl:hasOBONamespace>
        <oboInOwl:id>GAZ:00619924</oboInOwl:id>
        <rdfs:label>Kalkinsel</rdfs:label>
    </owl:NamedIndividual>
    


    <!-- http://purl.obolibrary.org/obo/GAZ_00621614 -->

    <owl:NamedIndividual rdf:about="http://purl.obolibrary.org/obo/GAZ_00621614">
        <obo:IAO_0000115>A canal.</obo:IAO_0000115>
        <oboInOwl:hasOBONamespace>GAZ</oboInOwl:hasOBONamespace>
        <oboInOwl:id>GAZ:00621614</oboInOwl:id>
        <rdfs:label>Muhlbach</rdfs:label>
    </owl:NamedIndividual>
    


    <!-- http://purl.obolibrary.org/obo/GAZ_00621615 -->

    <owl:NamedIndividual rdf:about="http://purl.obolibrary.org/obo/GAZ_00621615">
        <obo:IAO_0000115>A populated place. A region of Dachau.</obo:IAO_0000115>
        <oboInOwl:hasOBONamespace>GAZ</oboInOwl:hasOBONamespace>
        <oboInOwl:id>GAZ:00621615</oboInOwl:id>
        <rdfs:label>Schleissheimer Kanal</rdfs:label>
    </owl:NamedIndividual>
    


    <!-- http://purl.obolibrary.org/obo/GAZ_00622496 -->

    <owl:NamedIndividual rdf:about="http://purl.obolibrary.org/obo/GAZ_00622496">
        <obo:IAO_0000115>A hydroelectric power station.</obo:IAO_0000115>
        <oboInOwl:hasOBONamespace>GAZ</oboInOwl:hasOBONamespace>
        <oboInOwl:id>GAZ:00622496</oboInOwl:id>
        <rdfs:label>Kraftwerk Neufinsing</rdfs:label>
    </owl:NamedIndividual>
    


    <!-- http://purl.obolibrary.org/obo/GAZ_00622497 -->

    <owl:NamedIndividual rdf:about="http://purl.obolibrary.org/obo/GAZ_00622497">
        <obo:IAO_0000115>A hydroelectric power station.</obo:IAO_0000115>
        <oboInOwl:hasOBONamespace>GAZ</oboInOwl:hasOBONamespace>
        <oboInOwl:id>GAZ:00622497</oboInOwl:id>
        <rdfs:label>Speicherseekraftwerk Ismaning</rdfs:label>
    </owl:NamedIndividual>
    


    <!-- http://purl.obolibrary.org/obo/GAZ_00622498 -->

    <owl:NamedIndividual rdf:about="http://purl.obolibrary.org/obo/GAZ_00622498">
        <obo:IAO_0000115>A hydroelectric power station.</obo:IAO_0000115>
        <oboInOwl:hasOBONamespace>GAZ</oboInOwl:hasOBONamespace>
        <oboInOwl:id>GAZ:00622498</oboInOwl:id>
        <rdfs:label>Kraftwerk Aufkirchen</rdfs:label>
    </owl:NamedIndividual>
    


    <!-- http://purl.obolibrary.org/obo/GAZ_00622499 -->

    <owl:NamedIndividual rdf:about="http://purl.obolibrary.org/obo/GAZ_00622499">
        <obo:IAO_0000115>A hydroelectric power station.</obo:IAO_0000115>
        <oboInOwl:hasOBONamespace>GAZ</oboInOwl:hasOBONamespace>
        <oboInOwl:id>GAZ:00622499</oboInOwl:id>
        <rdfs:label>Kraftwerk Eitting</rdfs:label>
    </owl:NamedIndividual>
    


    <!-- http://purl.obolibrary.org/obo/GAZ_00622501 -->

    <owl:NamedIndividual rdf:about="http://purl.obolibrary.org/obo/GAZ_00622501">
        <obo:IAO_0000115>A river.</obo:IAO_0000115>
        <oboInOwl:hasOBONamespace>GAZ</oboInOwl:hasOBONamespace>
        <oboInOwl:id>GAZ:00622501</oboInOwl:id>
        <rdfs:label>Anzinger Sempt</rdfs:label>
    </owl:NamedIndividual>
    


    <!-- http://purl.obolibrary.org/obo/GAZ_00623318 -->

    <owl:NamedIndividual rdf:about="http://purl.obolibrary.org/obo/GAZ_00623318">
        <obo:IAO_0000115>A protected area.</obo:IAO_0000115>
        <oboInOwl:hasOBONamespace>GAZ</oboInOwl:hasOBONamespace>
        <oboInOwl:id>GAZ:00623318</oboInOwl:id>
        <rdfs:label>Vogelfreistatte Mittlere Isarstauseen</rdfs:label>
    </owl:NamedIndividual>
    


    <!-- http://purl.obolibrary.org/obo/GAZ_00623319 -->

    <owl:NamedIndividual rdf:about="http://purl.obolibrary.org/obo/GAZ_00623319">
        <obo:RO_0001025 rdf:resource="http://purl.obolibrary.org/obo/GAZ_00623318"/>
        <obo:IAO_0000115>Lakes.</obo:IAO_0000115>
        <oboInOwl:hasOBONamespace>GAZ</oboInOwl:hasOBONamespace>
        <oboInOwl:id>GAZ:00623319</oboInOwl:id>
        <rdfs:label>Isarstauseen</rdfs:label>
    </owl:NamedIndividual>
    


    <!-- http://purl.obolibrary.org/obo/GAZ_00623489 -->

    <owl:NamedIndividual rdf:about="http://purl.obolibrary.org/obo/GAZ_00623489">
        <obo:IAO_0000115>A hydroelectric power station.</obo:IAO_0000115>
        <oboInOwl:hasOBONamespace>GAZ</oboInOwl:hasOBONamespace>
        <oboInOwl:id>GAZ:00623489</oboInOwl:id>
        <rdfs:label>Wasserkraftwerk an der Ampe</rdfs:label>
    </owl:NamedIndividual>
    


    <!-- http://purl.obolibrary.org/obo/GAZ_00623580 -->

    <owl:NamedIndividual rdf:about="http://purl.obolibrary.org/obo/GAZ_00623580">
        <obo:IAO_0000115>A river.</obo:IAO_0000115>
        <oboInOwl:hasOBONamespace>GAZ</oboInOwl:hasOBONamespace>
        <oboInOwl:id>GAZ:00623580</oboInOwl:id>
        <rdfs:label>Stauwehr Krun</rdfs:label>
    </owl:NamedIndividual>
    


    <!-- http://purl.obolibrary.org/obo/GAZ_00623668 -->

    <owl:NamedIndividual rdf:about="http://purl.obolibrary.org/obo/GAZ_00623668">
        <obo:IAO_0000115>A weir.</obo:IAO_0000115>
        <oboInOwl:hasOBONamespace>GAZ</oboInOwl:hasOBONamespace>
        <oboInOwl:id>GAZ:00623668</oboInOwl:id>
        <rdfs:label>Karolinenwehr</rdfs:label>
    </owl:NamedIndividual>
    


    <!-- http://purl.obolibrary.org/obo/GAZ_00625635 -->

    <owl:NamedIndividual rdf:about="http://purl.obolibrary.org/obo/GAZ_00625635">
        <obo:IAO_0000115>A populated place. A City district (Stadtteil).</obo:IAO_0000115>
        <oboInOwl:hasOBONamespace>GAZ</oboInOwl:hasOBONamespace>
        <oboInOwl:id>GAZ:00625635</oboInOwl:id>
        <rdfs:label>Leopoldineninsel</rdfs:label>
    </owl:NamedIndividual>
    


    <!-- http://purl.obolibrary.org/obo/GAZ_00626162 -->

    <owl:NamedIndividual rdf:about="http://purl.obolibrary.org/obo/GAZ_00626162">
        <obo:IAO_0000115>A populated place. A district (Ortsteil).</obo:IAO_0000115>
        <oboInOwl:hasOBONamespace>GAZ</oboInOwl:hasOBONamespace>
        <oboInOwl:id>GAZ:00626162</oboInOwl:id>
        <rdfs:label>Leitzachwerke</rdfs:label>
    </owl:NamedIndividual>
    


    <!-- http://purl.obolibrary.org/obo/GAZ_00634202 -->

    <owl:NamedIndividual rdf:about="http://purl.obolibrary.org/obo/GAZ_00634202">
        <rdf:type rdf:resource="http://purl.obolibrary.org/obo/ENVO_00000423"/>
        <obo:IAO_0000115>A fluvial island.</obo:IAO_0000115>
        <oboInOwl:hasOBONamespace>GAZ</oboInOwl:hasOBONamespace>
        <oboInOwl:id>GAZ:00634202</oboInOwl:id>
        <rdfs:label>Untere Wohrd</rdfs:label>
    </owl:NamedIndividual>
    


    <!-- http://purl.obolibrary.org/obo/GAZ_00634203 -->

    <owl:NamedIndividual rdf:about="http://purl.obolibrary.org/obo/GAZ_00634203">
        <rdf:type rdf:resource="http://purl.obolibrary.org/obo/ENVO_00000423"/>
        <obo:IAO_0000115>A fluvial island.</obo:IAO_0000115>
        <oboInOwl:hasOBONamespace>GAZ</oboInOwl:hasOBONamespace>
        <oboInOwl:id>GAZ:00634203</oboInOwl:id>
        <rdfs:label>Obere Wohrd</rdfs:label>
    </owl:NamedIndividual>
    


    <!-- http://purl.obolibrary.org/obo/GAZ_00635331 -->

    <owl:NamedIndividual rdf:about="http://purl.obolibrary.org/obo/GAZ_00635331">
        <obo:IAO_0000115>A lake.</obo:IAO_0000115>
        <oboInOwl:hasOBONamespace>GAZ</oboInOwl:hasOBONamespace>
        <oboInOwl:id>GAZ:00635331</oboInOwl:id>
        <rdfs:label>Silbersee</rdfs:label>
    </owl:NamedIndividual>
    


    <!-- http://purl.obolibrary.org/obo/GAZ_00635572 -->

    <owl:NamedIndividual rdf:about="http://purl.obolibrary.org/obo/GAZ_00635572">
        <obo:IAO_0000115>A lock.</obo:IAO_0000115>
        <oboInOwl:hasOBONamespace>GAZ</oboInOwl:hasOBONamespace>
        <oboInOwl:id>GAZ:00635572</oboInOwl:id>
        <rdfs:label>Schleuse Bamberg</rdfs:label>
    </owl:NamedIndividual>
    


    <!-- http://purl.obolibrary.org/obo/GAZ_00635573 -->

    <owl:NamedIndividual rdf:about="http://purl.obolibrary.org/obo/GAZ_00635573">
        <obo:IAO_0000115>A lock.</obo:IAO_0000115>
        <oboInOwl:hasOBONamespace>GAZ</oboInOwl:hasOBONamespace>
        <oboInOwl:id>GAZ:00635573</oboInOwl:id>
        <rdfs:label>Schleuse Strullendorf</rdfs:label>
    </owl:NamedIndividual>
    


    <!-- http://purl.obolibrary.org/obo/GAZ_00635574 -->

    <owl:NamedIndividual rdf:about="http://purl.obolibrary.org/obo/GAZ_00635574">
        <obo:IAO_0000115>A lock.</obo:IAO_0000115>
        <oboInOwl:hasOBONamespace>GAZ</oboInOwl:hasOBONamespace>
        <oboInOwl:id>GAZ:00635574</oboInOwl:id>
        <rdfs:label>Schleuse Forchheim</rdfs:label>
    </owl:NamedIndividual>
    


    <!-- http://purl.obolibrary.org/obo/GAZ_00635575 -->

    <owl:NamedIndividual rdf:about="http://purl.obolibrary.org/obo/GAZ_00635575">
        <obo:IAO_0000115>A lock.</obo:IAO_0000115>
        <oboInOwl:hasOBONamespace>GAZ</oboInOwl:hasOBONamespace>
        <oboInOwl:id>GAZ:00635575</oboInOwl:id>
        <rdfs:label>Schleuse Hausen</rdfs:label>
    </owl:NamedIndividual>
    


    <!-- http://purl.obolibrary.org/obo/GAZ_00635576 -->

    <owl:NamedIndividual rdf:about="http://purl.obolibrary.org/obo/GAZ_00635576">
        <obo:IAO_0000115>A lock.</obo:IAO_0000115>
        <oboInOwl:hasOBONamespace>GAZ</oboInOwl:hasOBONamespace>
        <oboInOwl:id>GAZ:00635576</oboInOwl:id>
        <rdfs:label>Schleuse Erlangen</rdfs:label>
    </owl:NamedIndividual>
    


    <!-- http://purl.obolibrary.org/obo/GAZ_00635577 -->

    <owl:NamedIndividual rdf:about="http://purl.obolibrary.org/obo/GAZ_00635577">
        <obo:IAO_0000115>A lock.</obo:IAO_0000115>
        <oboInOwl:hasOBONamespace>GAZ</oboInOwl:hasOBONamespace>
        <oboInOwl:id>GAZ:00635577</oboInOwl:id>
        <rdfs:label>Schleuse Kriegenbrunn</rdfs:label>
    </owl:NamedIndividual>
    


    <!-- http://purl.obolibrary.org/obo/GAZ_00635578 -->

    <owl:NamedIndividual rdf:about="http://purl.obolibrary.org/obo/GAZ_00635578">
        <obo:IAO_0000115>A lock.</obo:IAO_0000115>
        <oboInOwl:hasOBONamespace>GAZ</oboInOwl:hasOBONamespace>
        <oboInOwl:id>GAZ:00635578</oboInOwl:id>
        <rdfs:label>Schleuse Nurnberg</rdfs:label>
    </owl:NamedIndividual>
    


    <!-- http://purl.obolibrary.org/obo/GAZ_00635579 -->

    <owl:NamedIndividual rdf:about="http://purl.obolibrary.org/obo/GAZ_00635579">
        <obo:IAO_0000115>A lock.</obo:IAO_0000115>
        <oboInOwl:hasOBONamespace>GAZ</oboInOwl:hasOBONamespace>
        <oboInOwl:id>GAZ:00635579</oboInOwl:id>
        <rdfs:label>Schleuse Eibach</rdfs:label>
    </owl:NamedIndividual>
    


    <!-- http://purl.obolibrary.org/obo/GAZ_00635580 -->

    <owl:NamedIndividual rdf:about="http://purl.obolibrary.org/obo/GAZ_00635580">
        <obo:IAO_0000115>A lock.</obo:IAO_0000115>
        <oboInOwl:hasOBONamespace>GAZ</oboInOwl:hasOBONamespace>
        <oboInOwl:id>GAZ:00635580</oboInOwl:id>
        <rdfs:label>Schleuse Eckersmuhlen</rdfs:label>
    </owl:NamedIndividual>
    


    <!-- http://purl.obolibrary.org/obo/GAZ_00635581 -->

    <owl:NamedIndividual rdf:about="http://purl.obolibrary.org/obo/GAZ_00635581">
        <obo:IAO_0000115>A lock.</obo:IAO_0000115>
        <oboInOwl:hasOBONamespace>GAZ</oboInOwl:hasOBONamespace>
        <oboInOwl:id>GAZ:00635581</oboInOwl:id>
        <rdfs:label>Schleuse Hilpoltstein</rdfs:label>
    </owl:NamedIndividual>
    


    <!-- http://purl.obolibrary.org/obo/GAZ_00635582 -->

    <owl:NamedIndividual rdf:about="http://purl.obolibrary.org/obo/GAZ_00635582">
        <obo:IAO_0000115>A lock.</obo:IAO_0000115>
        <oboInOwl:hasOBONamespace>GAZ</oboInOwl:hasOBONamespace>
        <oboInOwl:id>GAZ:00635582</oboInOwl:id>
        <rdfs:label>Schleuse Bachhausen</rdfs:label>
    </owl:NamedIndividual>
    


    <!-- http://purl.obolibrary.org/obo/GAZ_00635583 -->

    <owl:NamedIndividual rdf:about="http://purl.obolibrary.org/obo/GAZ_00635583">
        <obo:IAO_0000115>A populated place. A City district (Stadtteil).</obo:IAO_0000115>
        <oboInOwl:hasOBONamespace>GAZ</oboInOwl:hasOBONamespace>
        <oboInOwl:id>GAZ:00635583</oboInOwl:id>
        <rdfs:label>Schleuse Berching</rdfs:label>
    </owl:NamedIndividual>
    


    <!-- http://purl.obolibrary.org/obo/GAZ_00635584 -->

    <owl:NamedIndividual rdf:about="http://purl.obolibrary.org/obo/GAZ_00635584">
        <obo:IAO_0000115>A populated place. A City district (Stadtteil).</obo:IAO_0000115>
        <oboInOwl:hasOBONamespace>GAZ</oboInOwl:hasOBONamespace>
        <oboInOwl:id>GAZ:00635584</oboInOwl:id>
        <rdfs:label>Schleuse Dietfurt</rdfs:label>
    </owl:NamedIndividual>
    


    <!-- http://purl.obolibrary.org/obo/GAZ_00635585 -->

    <owl:NamedIndividual rdf:about="http://purl.obolibrary.org/obo/GAZ_00635585">
        <obo:IAO_0000115>A lock.</obo:IAO_0000115>
        <oboInOwl:hasOBONamespace>GAZ</oboInOwl:hasOBONamespace>
        <oboInOwl:id>GAZ:00635585</oboInOwl:id>
        <rdfs:label>Schleuse Riedenburg</rdfs:label>
    </owl:NamedIndividual>
    


    <!-- http://purl.obolibrary.org/obo/GAZ_00635586 -->

    <owl:NamedIndividual rdf:about="http://purl.obolibrary.org/obo/GAZ_00635586">
        <obo:IAO_0000115>A lock.</obo:IAO_0000115>
        <oboInOwl:hasOBONamespace>GAZ</oboInOwl:hasOBONamespace>
        <oboInOwl:id>GAZ:00635586</oboInOwl:id>
        <rdfs:label>Schleuse Kelheim</rdfs:label>
    </owl:NamedIndividual>
    


    <!-- http://purl.obolibrary.org/obo/GAZ_00635589 -->

    <owl:NamedIndividual rdf:about="http://purl.obolibrary.org/obo/GAZ_00635589">
        <obo:IAO_0000115>An island; a protected area.</obo:IAO_0000115>
        <oboInOwl:hasOBONamespace>GAZ</oboInOwl:hasOBONamespace>
        <oboInOwl:id>GAZ:00635589</oboInOwl:id>
        <rdfs:label>Vogelfreistatte Flachwasser- und Inselzone im Altmuhlsee</rdfs:label>
    </owl:NamedIndividual>
    


    <!-- http://purl.obolibrary.org/obo/GAZ_00635860 -->

    <owl:NamedIndividual rdf:about="http://purl.obolibrary.org/obo/GAZ_00635860">
        <obo:IAO_0000115>A river.</obo:IAO_0000115>
        <oboInOwl:hasOBONamespace>GAZ</oboInOwl:hasOBONamespace>
        <oboInOwl:id>GAZ:00635860</oboInOwl:id>
        <rdfs:label>Urtlbach</rdfs:label>
    </owl:NamedIndividual>
    


    <!-- http://purl.obolibrary.org/obo/GAZ_00637654 -->

    <owl:NamedIndividual rdf:about="http://purl.obolibrary.org/obo/GAZ_00637654">
        <obo:IAO_0000115>A reservoir.</obo:IAO_0000115>
        <oboInOwl:hasOBONamespace>GAZ</oboInOwl:hasOBONamespace>
        <oboInOwl:id>GAZ:00637654</oboInOwl:id>
        <rdfs:label>Perlsee [lake]</rdfs:label>
    </owl:NamedIndividual>
    


    <!-- http://purl.obolibrary.org/obo/GAZ_00637942 -->

    <owl:NamedIndividual rdf:about="http://purl.obolibrary.org/obo/GAZ_00637942">
        <obo:IAO_0000115>A populated place. A district (Ortsteil).</obo:IAO_0000115>
        <oboInOwl:hasOBONamespace>GAZ</oboInOwl:hasOBONamespace>
        <oboInOwl:id>GAZ:00637942</oboInOwl:id>
        <rdfs:label>Trausnitztalsperre</rdfs:label>
    </owl:NamedIndividual>
    


    <!-- http://purl.obolibrary.org/obo/GAZ_00644175 -->

    <owl:NamedIndividual rdf:about="http://purl.obolibrary.org/obo/GAZ_00644175">
        <obo:IAO_0000115>A lake.</obo:IAO_0000115>
        <oboInOwl:hasOBONamespace>GAZ</oboInOwl:hasOBONamespace>
        <oboInOwl:id>GAZ:00644175</oboInOwl:id>
        <rdfs:label>Hartsfeldsee</rdfs:label>
    </owl:NamedIndividual>
    


    <!-- http://purl.obolibrary.org/obo/GAZ_00644704 -->

    <owl:NamedIndividual rdf:about="http://purl.obolibrary.org/obo/GAZ_00644704">
        <obo:IAO_0000115>A river.</obo:IAO_0000115>
        <oboInOwl:hasOBONamespace>GAZ</oboInOwl:hasOBONamespace>
        <oboInOwl:id>GAZ:00644704</oboInOwl:id>
        <rdfs:label>Hungerbach</rdfs:label>
    </owl:NamedIndividual>
    


    <!-- http://purl.obolibrary.org/obo/GAZ_00644705 -->

    <owl:NamedIndividual rdf:about="http://purl.obolibrary.org/obo/GAZ_00644705">
        <obo:IAO_0000115>A river.</obo:IAO_0000115>
        <oboInOwl:hasOBONamespace>GAZ</oboInOwl:hasOBONamespace>
        <oboInOwl:id>GAZ:00644705</oboInOwl:id>
        <rdfs:label>Schnittenbach</rdfs:label>
    </owl:NamedIndividual>
    


    <!-- http://purl.obolibrary.org/obo/GAZ_00644706 -->

    <owl:NamedIndividual rdf:about="http://purl.obolibrary.org/obo/GAZ_00644706">
        <obo:IAO_0000115>A river.</obo:IAO_0000115>
        <oboInOwl:hasOBONamespace>GAZ</oboInOwl:hasOBONamespace>
        <oboInOwl:id>GAZ:00644706</oboInOwl:id>
        <rdfs:label>Kohbach</rdfs:label>
    </owl:NamedIndividual>
    


    <!-- http://purl.obolibrary.org/obo/GAZ_00644740 -->

    <owl:NamedIndividual rdf:about="http://purl.obolibrary.org/obo/GAZ_00644740">
        <obo:IAO_0000115>A lake.</obo:IAO_0000115>
        <oboInOwl:hasOBONamespace>GAZ</oboInOwl:hasOBONamespace>
        <oboInOwl:id>GAZ:00644740</oboInOwl:id>
        <rdfs:label>Fuggerweihe</rdfs:label>
    </owl:NamedIndividual>
    


    <!-- http://purl.obolibrary.org/obo/GAZ_00645442 -->

    <owl:NamedIndividual rdf:about="http://purl.obolibrary.org/obo/GAZ_00645442">
        <rdf:type rdf:resource="http://purl.obolibrary.org/obo/ENVO_00000423"/>
        <obo:IAO_0000115>A fluvial island.</obo:IAO_0000115>
        <oboInOwl:hasOBONamespace>GAZ</oboInOwl:hasOBONamespace>
        <oboInOwl:id>GAZ:00645442</oboInOwl:id>
        <rdfs:label>Georgsinsel</rdfs:label>
    </owl:NamedIndividual>
    


    <!-- http://purl.obolibrary.org/obo/GAZ_00645872 -->

    <owl:NamedIndividual rdf:about="http://purl.obolibrary.org/obo/GAZ_00645872">
        <obo:IAO_0000115>A hydroelectric power plant.</obo:IAO_0000115>
        <oboInOwl:hasOBONamespace>GAZ</oboInOwl:hasOBONamespace>
        <oboInOwl:id>GAZ:00645872</oboInOwl:id>
        <rdfs:label>Kleinstkraftwerk Kirnach</rdfs:label>
    </owl:NamedIndividual>
    


    <!-- http://purl.obolibrary.org/obo/GAZ_00646554 -->

    <owl:NamedIndividual rdf:about="http://purl.obolibrary.org/obo/GAZ_00646554">
        <obo:IAO_0000115>A harbor.</obo:IAO_0000115>
        <oboInOwl:hasOBONamespace>GAZ</oboInOwl:hasOBONamespace>
        <oboInOwl:id>GAZ:00646554</oboInOwl:id>
        <rdfs:label>Bayernhafen Nurnberg</rdfs:label>
    </owl:NamedIndividual>
    


    <!-- http://purl.obolibrary.org/obo/GAZ_00646556 -->

    <owl:NamedIndividual rdf:about="http://purl.obolibrary.org/obo/GAZ_00646556">
        <obo:IAO_0000115>A harbor.</obo:IAO_0000115>
        <oboInOwl:hasOBONamespace>GAZ</oboInOwl:hasOBONamespace>
        <oboInOwl:id>GAZ:00646556</oboInOwl:id>
        <rdfs:label>Bayernhafen Regensburg</rdfs:label>
    </owl:NamedIndividual>
    


    <!-- http://purl.obolibrary.org/obo/GAZ_00646557 -->

    <owl:NamedIndividual rdf:about="http://purl.obolibrary.org/obo/GAZ_00646557">
        <obo:IAO_0000115>A harbor.</obo:IAO_0000115>
        <oboInOwl:hasOBONamespace>GAZ</oboInOwl:hasOBONamespace>
        <oboInOwl:id>GAZ:00646557</oboInOwl:id>
        <rdfs:label>Bayernhafen Passau</rdfs:label>
    </owl:NamedIndividual>
    


    <!-- http://purl.obolibrary.org/obo/GAZ_00648958 -->

    <owl:NamedIndividual rdf:about="http://purl.obolibrary.org/obo/GAZ_00648958">
        <obo:IAO_0000115>A river.</obo:IAO_0000115>
        <oboInOwl:hasOBONamespace>GAZ</oboInOwl:hasOBONamespace>
        <oboInOwl:id>GAZ:00648958</oboInOwl:id>
        <rdfs:label>Halsbach</rdfs:label>
    </owl:NamedIndividual>
    


    <!-- http://purl.obolibrary.org/obo/GAZ_00648967 -->

    <owl:NamedIndividual rdf:about="http://purl.obolibrary.org/obo/GAZ_00648967">
        <obo:IAO_0000115>A pumped-storage power station.</obo:IAO_0000115>
        <oboInOwl:hasOBONamespace>GAZ</oboInOwl:hasOBONamespace>
        <oboInOwl:id>GAZ:00648967</oboInOwl:id>
        <rdfs:label>Pumpspeicherkraftwerk Ranna</rdfs:label>
    </owl:NamedIndividual>
    


    <!-- http://purl.obolibrary.org/obo/GAZ_00648981 -->

    <owl:NamedIndividual rdf:about="http://purl.obolibrary.org/obo/GAZ_00648981">
        <obo:IAO_0000115>A river.</obo:IAO_0000115>
        <oboInOwl:hasOBONamespace>GAZ</oboInOwl:hasOBONamespace>
        <oboInOwl:id>GAZ:00648981</oboInOwl:id>
        <rdfs:label>Krebsbach</rdfs:label>
    </owl:NamedIndividual>
    


    <!-- http://purl.obolibrary.org/obo/GAZ_00649195 -->

    <owl:NamedIndividual rdf:about="http://purl.obolibrary.org/obo/GAZ_00649195">
        <obo:IAO_0000115>A hydroelectric power station.</obo:IAO_0000115>
        <oboInOwl:hasOBONamespace>GAZ</oboInOwl:hasOBONamespace>
        <oboInOwl:id>GAZ:00649195</oboInOwl:id>
        <rdfs:label>Kraftwerk Bad Abbach</rdfs:label>
    </owl:NamedIndividual>
    


    <!-- http://purl.obolibrary.org/obo/GAZ_00650219 -->

    <owl:NamedIndividual rdf:about="http://purl.obolibrary.org/obo/GAZ_00650219">
        <obo:IAO_0000115>A populated place. A district (Ortsteil).</obo:IAO_0000115>
        <oboInOwl:hasOBONamespace>GAZ</oboInOwl:hasOBONamespace>
        <oboInOwl:id>GAZ:00650219</oboInOwl:id>
        <rdfs:label>Kanalschleuse 28</rdfs:label>
    </owl:NamedIndividual>
    


    <!-- http://purl.obolibrary.org/obo/GAZ_00650220 -->

    <owl:NamedIndividual rdf:about="http://purl.obolibrary.org/obo/GAZ_00650220">
        <obo:IAO_0000115>A populated place. A district (Ortsteil).</obo:IAO_0000115>
        <oboInOwl:hasOBONamespace>GAZ</oboInOwl:hasOBONamespace>
        <oboInOwl:id>GAZ:00650220</oboInOwl:id>
        <rdfs:label>Kanalschleuse 29</rdfs:label>
    </owl:NamedIndividual>
    


    <!-- http://purl.obolibrary.org/obo/GAZ_00650221 -->

    <owl:NamedIndividual rdf:about="http://purl.obolibrary.org/obo/GAZ_00650221">
        <obo:IAO_0000115>A populated place. A district (Ortsteil).</obo:IAO_0000115>
        <oboInOwl:hasOBONamespace>GAZ</oboInOwl:hasOBONamespace>
        <oboInOwl:id>GAZ:00650221</oboInOwl:id>
        <rdfs:label>Kanalschleuse 30</rdfs:label>
    </owl:NamedIndividual>
    


    <!-- http://purl.obolibrary.org/obo/GAZ_00650670 -->

    <owl:NamedIndividual rdf:about="http://purl.obolibrary.org/obo/GAZ_00650670">
        <obo:IAO_0000115>A river.</obo:IAO_0000115>
        <oboInOwl:hasOBONamespace>GAZ</oboInOwl:hasOBONamespace>
        <oboInOwl:id>GAZ:00650670</oboInOwl:id>
        <rdfs:label>Angerbach</rdfs:label>
    </owl:NamedIndividual>
    


    <!-- http://purl.obolibrary.org/obo/GAZ_00650671 -->

    <owl:NamedIndividual rdf:about="http://purl.obolibrary.org/obo/GAZ_00650671">
        <obo:IAO_0000115>A river.</obo:IAO_0000115>
        <oboInOwl:hasOBONamespace>GAZ</oboInOwl:hasOBONamespace>
        <oboInOwl:id>GAZ:00650671</oboInOwl:id>
        <rdfs:label>Grosskristenbach</rdfs:label>
    </owl:NamedIndividual>
    


    <!-- http://purl.obolibrary.org/obo/GAZ_00650673 -->

    <owl:NamedIndividual rdf:about="http://purl.obolibrary.org/obo/GAZ_00650673">
        <obo:IAO_0000115>A river.</obo:IAO_0000115>
        <oboInOwl:hasOBONamespace>GAZ</oboInOwl:hasOBONamespace>
        <oboInOwl:id>GAZ:00650673</oboInOwl:id>
        <rdfs:label>Reschenbach</rdfs:label>
    </owl:NamedIndividual>
    


    <!-- http://purl.obolibrary.org/obo/GAZ_00650735 -->

    <owl:NamedIndividual rdf:about="http://purl.obolibrary.org/obo/GAZ_00650735">
        <obo:IAO_0000115>A river.</obo:IAO_0000115>
        <oboInOwl:hasOBONamespace>GAZ</oboInOwl:hasOBONamespace>
        <oboInOwl:id>GAZ:00650735</oboInOwl:id>
        <rdfs:label>Weissbach [Lattengebirge]</rdfs:label>
    </owl:NamedIndividual>
    


    <!-- http://purl.obolibrary.org/obo/GAZ_00650849 -->

    <owl:NamedIndividual rdf:about="http://purl.obolibrary.org/obo/GAZ_00650849">
        <obo:IAO_0000115>A river of Bavaria, Germany.</obo:IAO_0000115>
        <oboInOwl:hasOBONamespace>GAZ</oboInOwl:hasOBONamespace>
        <oboInOwl:id>GAZ:00650849</oboInOwl:id>
        <rdfs:label>Mailinger Bach</rdfs:label>
    </owl:NamedIndividual>
    


    <!-- http://purl.obolibrary.org/obo/GAZ_00650850 -->

    <owl:NamedIndividual rdf:about="http://purl.obolibrary.org/obo/GAZ_00650850">
        <obo:RO_0001025 rdf:resource="http://purl.obolibrary.org/obo/GAZ_00650849"/>
        <obo:IAO_0000115>A river.</obo:IAO_0000115>
        <oboInOwl:hasOBONamespace>GAZ</oboInOwl:hasOBONamespace>
        <oboInOwl:id>GAZ:00650850</oboInOwl:id>
        <rdfs:label>Gussgraben</rdfs:label>
    </owl:NamedIndividual>
    


    <!-- http://purl.obolibrary.org/obo/GAZ_00650851 -->

    <owl:NamedIndividual rdf:about="http://purl.obolibrary.org/obo/GAZ_00650851">
        <obo:RO_0001025 rdf:resource="http://purl.obolibrary.org/obo/GAZ_00650849"/>
        <obo:IAO_0000115>A river.</obo:IAO_0000115>
        <oboInOwl:hasOBONamespace>GAZ</oboInOwl:hasOBONamespace>
        <oboInOwl:id>GAZ:00650851</oboInOwl:id>
        <rdfs:label>Zellaugraben</rdfs:label>
    </owl:NamedIndividual>
    


    <!-- http://purl.obolibrary.org/obo/GAZ_00650852 -->

    <owl:NamedIndividual rdf:about="http://purl.obolibrary.org/obo/GAZ_00650852">
        <obo:RO_0001025 rdf:resource="http://purl.obolibrary.org/obo/GAZ_00650849"/>
        <obo:IAO_0000115>A river.</obo:IAO_0000115>
        <oboInOwl:hasOBONamespace>GAZ</oboInOwl:hasOBONamespace>
        <oboInOwl:id>GAZ:00650852</oboInOwl:id>
        <rdfs:label>Augraben</rdfs:label>
    </owl:NamedIndividual>
    


    <!-- http://purl.obolibrary.org/obo/GAZ_00650853 -->

    <owl:NamedIndividual rdf:about="http://purl.obolibrary.org/obo/GAZ_00650853">
        <obo:RO_0001025 rdf:resource="http://purl.obolibrary.org/obo/GAZ_00650849"/>
        <obo:IAO_0000115>A river.</obo:IAO_0000115>
        <oboInOwl:hasOBONamespace>GAZ</oboInOwl:hasOBONamespace>
        <oboInOwl:id>GAZ:00650853</oboInOwl:id>
        <rdfs:label>Koschinger Bach</rdfs:label>
    </owl:NamedIndividual>
    


    <!-- http://purl.obolibrary.org/obo/GAZ_00650863 -->

    <owl:NamedIndividual rdf:about="http://purl.obolibrary.org/obo/GAZ_00650863">
        <obo:IAO_0000115>A river of Bavaria, Germany.</obo:IAO_0000115>
        <oboInOwl:hasOBONamespace>GAZ</oboInOwl:hasOBONamespace>
        <oboInOwl:id>GAZ:00650863</oboInOwl:id>
        <rdfs:label>Giessgraben</rdfs:label>
    </owl:NamedIndividual>
    


    <!-- http://purl.obolibrary.org/obo/GAZ_00650864 -->

    <owl:NamedIndividual rdf:about="http://purl.obolibrary.org/obo/GAZ_00650864">
        <obo:IAO_0000115>A karst spring.</obo:IAO_0000115>
        <oboInOwl:hasOBONamespace>GAZ</oboInOwl:hasOBONamespace>
        <oboInOwl:id>GAZ:00650864</oboInOwl:id>
        <rdfs:label>Glessbrunnen</rdfs:label>
    </owl:NamedIndividual>
    


    <!-- http://purl.obolibrary.org/obo/GAZ_00651135 -->

    <owl:NamedIndividual rdf:about="http://purl.obolibrary.org/obo/GAZ_00651135">
        <obo:IAO_0000115>A hydroelectric power station.</obo:IAO_0000115>
        <oboInOwl:hasOBONamespace>GAZ</oboInOwl:hasOBONamespace>
        <oboInOwl:id>GAZ:00651135</oboInOwl:id>
        <rdfs:label>Wasserkraftwerk Muhltal</rdfs:label>
    </owl:NamedIndividual>
    


    <!-- http://purl.obolibrary.org/obo/GAZ_00651154 -->

    <owl:NamedIndividual rdf:about="http://purl.obolibrary.org/obo/GAZ_00651154">
        <obo:IAO_0000115>A hydroelectric power station.</obo:IAO_0000115>
        <oboInOwl:hasOBONamespace>GAZ</oboInOwl:hasOBONamespace>
        <oboInOwl:id>GAZ:00651154</oboInOwl:id>
        <rdfs:label>Kraftwerk Pulling</rdfs:label>
    </owl:NamedIndividual>
    


    <!-- http://purl.obolibrary.org/obo/GAZ_00651155 -->

    <owl:NamedIndividual rdf:about="http://purl.obolibrary.org/obo/GAZ_00651155">
        <obo:IAO_0000115>A canal; an annabranch of the Danube.</obo:IAO_0000115>
        <oboInOwl:hasOBONamespace>GAZ</oboInOwl:hasOBONamespace>
        <oboInOwl:id>GAZ:00651155</oboInOwl:id>
        <rdfs:label>Europakanal</rdfs:label>
    </owl:NamedIndividual>
    


    <!-- http://purl.obolibrary.org/obo/GAZ_00653715 -->

    <owl:NamedIndividual rdf:about="http://purl.obolibrary.org/obo/GAZ_00653715">
        <obo:IAO_0000115>A hydroelectric power station.</obo:IAO_0000115>
        <oboInOwl:hasOBONamespace>GAZ</oboInOwl:hasOBONamespace>
        <oboInOwl:id>GAZ:00653715</oboInOwl:id>
        <rdfs:label>Wasserkraftwerk Dingolfing</rdfs:label>
    </owl:NamedIndividual>
    


    <!-- 
    ///////////////////////////////////////////////////////////////////////////////////////
    //
    // Annotations
    //
    ///////////////////////////////////////////////////////////////////////////////////////
     -->

    <rdf:Description rdf:about="http://purl.obolibrary.org/obo/GAZ_00003594">
        <oboInOwl:id>GAZ:00003594</oboInOwl:id>
        <rdfs:label>Region (Hungary)</rdfs:label>
        <oboInOwl:hasOBONamespace>GAZ</oboInOwl:hasOBONamespace>
    </rdf:Description>
    <rdf:Description rdf:about="http://purl.obolibrary.org/obo/GAZ_00003595">
        <oboInOwl:id>GAZ:00003595</oboInOwl:id>
        <rdfs:label>Central Hungary</rdfs:label>
        <oboInOwl:hasOBONamespace>GAZ</oboInOwl:hasOBONamespace>
    </rdf:Description>
    <rdf:Description rdf:about="http://purl.obolibrary.org/obo/GAZ_00003596">
        <rdfs:label>Central Transdanubia</rdfs:label>
        <oboInOwl:id>GAZ:00003596</oboInOwl:id>
        <oboInOwl:hasOBONamespace>GAZ</oboInOwl:hasOBONamespace>
    </rdf:Description>
    <rdf:Description rdf:about="http://purl.obolibrary.org/obo/GAZ_00003597">
        <oboInOwl:id>GAZ:00003597</oboInOwl:id>
        <rdfs:label>Northern Great Plain</rdfs:label>
        <oboInOwl:hasOBONamespace>GAZ</oboInOwl:hasOBONamespace>
    </rdf:Description>
    <rdf:Description rdf:about="http://purl.obolibrary.org/obo/GAZ_00003598">
        <oboInOwl:hasOBONamespace>GAZ</oboInOwl:hasOBONamespace>
        <rdfs:label>Western Transdanubia</rdfs:label>
        <oboInOwl:id>GAZ:00003598</oboInOwl:id>
    </rdf:Description>
    <rdf:Description rdf:about="http://purl.obolibrary.org/obo/GAZ_00003599">
        <oboInOwl:hasOBONamespace>GAZ</oboInOwl:hasOBONamespace>
        <oboInOwl:id>GAZ:00003599</oboInOwl:id>
        <rdfs:label>Southern Great Plain</rdfs:label>
    </rdf:Description>
    <rdf:Description rdf:about="http://purl.obolibrary.org/obo/GAZ_00003600">
        <rdfs:label>Southern Transdanubia</rdfs:label>
        <oboInOwl:id>GAZ:00003600</oboInOwl:id>
        <oboInOwl:hasOBONamespace>GAZ</oboInOwl:hasOBONamespace>
    </rdf:Description>
    <rdf:Description rdf:about="http://purl.obolibrary.org/obo/GAZ_00003601">
        <rdfs:label>Northern Hungary</rdfs:label>
        <oboInOwl:id>GAZ:00003601</oboInOwl:id>
        <oboInOwl:hasOBONamespace>GAZ</oboInOwl:hasOBONamespace>
    </rdf:Description>
    <rdf:Description rdf:about="http://purl.obolibrary.org/obo/GAZ_00003602">
        <rdfs:label>Tihany</rdfs:label>
        <oboInOwl:id>GAZ:00003602</oboInOwl:id>
        <oboInOwl:hasOBONamespace>GAZ</oboInOwl:hasOBONamespace>
        <obo:IAO_0000115>A populated place. A village on the northern shore of Lake Balaton on the Tihany Peninsula.</obo:IAO_0000115>
    </rdf:Description>
    <rdf:Description rdf:about="http://purl.obolibrary.org/obo/GAZ_00003603">
        <oboInOwl:hasOBONamespace>GAZ</oboInOwl:hasOBONamespace>
        <rdfs:label>populated place, Hungary</rdfs:label>
        <oboInOwl:id>GAZ:00003603</oboInOwl:id>
    </rdf:Description>
    <rdf:Description rdf:about="http://purl.obolibrary.org/obo/GAZ_00004702">
        <oboInOwl:id>GAZ:00004702</oboInOwl:id>
        <oboInOwl:hasOBONamespace>GAZ</oboInOwl:hasOBONamespace>
        <rdfs:label>Tatabanya</rdfs:label>
    </rdf:Description>
    <rdf:Description rdf:about="http://purl.obolibrary.org/obo/GAZ_00008479">
        <oboInOwl:id>GAZ:00008479</oboInOwl:id>
        <rdfs:label>Paloznak</rdfs:label>
        <oboInOwl:hasOBONamespace>GAZ</oboInOwl:hasOBONamespace>
    </rdf:Description>
    <rdf:Description rdf:about="http://purl.obolibrary.org/obo/GAZ_00010080">
        <rdfs:label>Hodmezovasarhely</rdfs:label>
        <oboInOwl:hasOBONamespace>GAZ</oboInOwl:hasOBONamespace>
        <oboInOwl:id>GAZ:00010080</oboInOwl:id>
    </rdf:Description>
    <rdf:Description rdf:about="http://purl.obolibrary.org/obo/GAZ_00036861">
        <rdfs:label>Budapest</rdfs:label>
        <oboInOwl:hasOBONamespace>GAZ</oboInOwl:hasOBONamespace>
        <oboInOwl:id>GAZ:00036861</oboInOwl:id>
    </rdf:Description>
    <rdf:Description rdf:about="http://purl.obolibrary.org/obo/GAZ_00043965">
        <oboInOwl:id>GAZ:00043965</oboInOwl:id>
        <rdfs:label>Esztergom</rdfs:label>
        <oboInOwl:hasOBONamespace>GAZ</oboInOwl:hasOBONamespace>
    </rdf:Description>
    <rdf:Description rdf:about="http://purl.obolibrary.org/obo/GAZ_00103879">
        <rdfs:label>Agasegyhaza</rdfs:label>
        <oboInOwl:id>GAZ:00103879</oboInOwl:id>
        <obo:IAO_0000115>A populated place. A village in Bacs-Kiskun county, in the Southern Great Plain region of southern Hungary.</obo:IAO_0000115>
        <oboInOwl:hasOBONamespace>GAZ</oboInOwl:hasOBONamespace>
    </rdf:Description>
    <rdf:Description rdf:about="http://purl.obolibrary.org/obo/GAZ_00148095">
        <obo:IAO_0000115>Artificial water reservoirs in the Stiavnica Mountains, in central Slovakia. Most of them were built in order to provide energy for the silver mines of Banska Stiavnica in the 18th century. At their height, tajchy comprised a sophisticated system of 60 reservoirs, connected to each other by more than 100 km of channels and underground tunnels. 24 artificial lakes still exist. They consititute a World Heritage Site.</obo:IAO_0000115>
        <oboInOwl:hasOBONamespace>GAZ</oboInOwl:hasOBONamespace>
        <oboInOwl:id>GAZ:00148095</oboInOwl:id>
        <rdfs:label>Tajchy</rdfs:label>
    </rdf:Description>
    <rdf:Description rdf:about="http://purl.obolibrary.org/obo/GAZ_00148096">
        <obo:IAO_0000115>A tajch.</obo:IAO_0000115>
        <oboInOwl:hasOBONamespace>GAZ</oboInOwl:hasOBONamespace>
        <oboInOwl:id>GAZ:00148096</oboInOwl:id>
        <rdfs:label>Pocuvadlianske jazeroin</rdfs:label>
    </rdf:Description>
    <rdf:Description rdf:about="http://purl.obolibrary.org/obo/GAZ_00148097">
        <obo:IAO_0000115>A tajch.</obo:IAO_0000115>
        <oboInOwl:id>GAZ:00148097</oboInOwl:id>
        <rdfs:label>Lintisske jazero</rdfs:label>
        <oboInOwl:hasOBONamespace>GAZ</oboInOwl:hasOBONamespace>
    </rdf:Description>
    <rdf:Description rdf:about="http://purl.obolibrary.org/obo/GAZ_00148098">
        <oboInOwl:id>GAZ:00148098</oboInOwl:id>
        <obo:IAO_0000115>A tajch.</obo:IAO_0000115>
        <oboInOwl:hasOBONamespace>GAZ</oboInOwl:hasOBONamespace>
        <rdfs:label>Jazero Klinger</rdfs:label>
    </rdf:Description>
    <rdf:Description rdf:about="http://purl.obolibrary.org/obo/GAZ_00148099">
        <obo:IAO_0000115>A tajch.</obo:IAO_0000115>
        <rdfs:label>Jazero Bakomi</rdfs:label>
        <oboInOwl:hasOBONamespace>GAZ</oboInOwl:hasOBONamespace>
        <oboInOwl:id>GAZ:00148099</oboInOwl:id>
    </rdf:Description>
    <rdf:Description rdf:about="http://purl.obolibrary.org/obo/GAZ_00148100">
        <oboInOwl:hasOBONamespace>GAZ</oboInOwl:hasOBONamespace>
        <rdfs:label>Belianske jazero</rdfs:label>
        <oboInOwl:id>GAZ:00148100</oboInOwl:id>
        <obo:IAO_0000115>A tajch.</obo:IAO_0000115>
    </rdf:Description>
    <rdf:Description rdf:about="http://purl.obolibrary.org/obo/GAZ_00148101">
        <oboInOwl:hasOBONamespace>GAZ</oboInOwl:hasOBONamespace>
        <obo:IAO_0000115>A tajch.</obo:IAO_0000115>
        <rdfs:label>Krechsengrundske jazero</rdfs:label>
        <oboInOwl:id>GAZ:00148101</oboInOwl:id>
    </rdf:Description>
    <rdf:Description rdf:about="http://purl.obolibrary.org/obo/GAZ_00148102">
        <oboInOwl:hasOBONamespace>GAZ</oboInOwl:hasOBONamespace>
        <rdfs:label>Jazero Cervena studna</rdfs:label>
        <obo:IAO_0000115>A tajch.</obo:IAO_0000115>
        <oboInOwl:id>GAZ:00148102</oboInOwl:id>
    </rdf:Description>
    <rdf:Description rdf:about="http://purl.obolibrary.org/obo/GAZ_00148103">
        <oboInOwl:hasOBONamespace>GAZ</oboInOwl:hasOBONamespace>
        <rdfs:label>Kolpaeske ve&apos;ke jazero</rdfs:label>
        <oboInOwl:id>GAZ:00148103</oboInOwl:id>
        <obo:IAO_0000115>A tajch.</obo:IAO_0000115>
    </rdf:Description>
    <rdf:Description rdf:about="http://purl.obolibrary.org/obo/GAZ_00148104">
        <oboInOwl:hasOBONamespace>GAZ</oboInOwl:hasOBONamespace>
        <oboInOwl:id>GAZ:00148104</oboInOwl:id>
        <rdfs:label>Halcianske jazero</rdfs:label>
        <obo:IAO_0000115>A tajch.</obo:IAO_0000115>
    </rdf:Description>
    <rdf:Description rdf:about="http://purl.obolibrary.org/obo/GAZ_00148105">
        <rdfs:label>Kysihyblianske jazera</rdfs:label>
        <oboInOwl:id>GAZ:00148105</oboInOwl:id>
        <obo:IAO_0000115>A tajch.</obo:IAO_0000115>
        <oboInOwl:hasOBONamespace>GAZ</oboInOwl:hasOBONamespace>
    </rdf:Description>
    <rdf:Description rdf:about="http://purl.obolibrary.org/obo/GAZ_00148106">
        <rdfs:label>Goldfuzske jazero</rdfs:label>
        <oboInOwl:id>GAZ:00148106</oboInOwl:id>
        <oboInOwl:hasOBONamespace>GAZ</oboInOwl:hasOBONamespace>
        <obo:IAO_0000115>A tajch.</obo:IAO_0000115>
    </rdf:Description>
    <rdf:Description rdf:about="http://purl.obolibrary.org/obo/GAZ_00148107">
        <oboInOwl:id>GAZ:00148107</oboInOwl:id>
        <oboInOwl:hasOBONamespace>GAZ</oboInOwl:hasOBONamespace>
        <obo:IAO_0000115>A tajch.</obo:IAO_0000115>
        <rdfs:label>Kolpasske male jazero</rdfs:label>
    </rdf:Description>
    <rdf:Description rdf:about="http://purl.obolibrary.org/obo/GAZ_00148108">
        <oboInOwl:hasOBONamespace>GAZ</oboInOwl:hasOBONamespace>
        <oboInOwl:id>GAZ:00148108</oboInOwl:id>
        <rdfs:label>Evickino jazero</rdfs:label>
        <obo:IAO_0000115>A tajch.</obo:IAO_0000115>
    </rdf:Description>
    <rdf:Description rdf:about="http://purl.obolibrary.org/obo/GAZ_00148109">
        <oboInOwl:id>GAZ:00148109</oboInOwl:id>
        <rdfs:label>Michelstolnianske jazero</rdfs:label>
        <oboInOwl:hasOBONamespace>GAZ</oboInOwl:hasOBONamespace>
        <obo:IAO_0000115>A tajch.</obo:IAO_0000115>
    </rdf:Description>
    <rdf:Description rdf:about="http://purl.obolibrary.org/obo/GAZ_00148110">
        <obo:IAO_0000115>A tajch.</obo:IAO_0000115>
        <oboInOwl:hasOBONamespace>GAZ</oboInOwl:hasOBONamespace>
        <oboInOwl:id>GAZ:00148110</oboInOwl:id>
        <rdfs:label>Samposske jazero</rdfs:label>
    </rdf:Description>
    <rdf:Description rdf:about="http://purl.obolibrary.org/obo/GAZ_00148111">
        <oboInOwl:hasOBONamespace>GAZ</oboInOwl:hasOBONamespace>
        <obo:IAO_0000115>A tajch.</obo:IAO_0000115>
        <oboInOwl:id>GAZ:00148111</oboInOwl:id>
        <rdfs:label>Vodarenske ve&apos;ke jazero</rdfs:label>
    </rdf:Description>
    <rdf:Description rdf:about="http://purl.obolibrary.org/obo/GAZ_00148112">
        <rdfs:label>Ottergrundskw jazero</rdfs:label>
        <oboInOwl:hasOBONamespace>GAZ</oboInOwl:hasOBONamespace>
        <obo:IAO_0000115>A tajch.</obo:IAO_0000115>
        <oboInOwl:id>GAZ:00148112</oboInOwl:id>
    </rdf:Description>
    <rdf:Description rdf:about="http://purl.obolibrary.org/obo/GAZ_00148113">
        <oboInOwl:hasOBONamespace>GAZ</oboInOwl:hasOBONamespace>
        <rdfs:label>Rozgrundske jazero</rdfs:label>
        <obo:IAO_0000115>A tajch.</obo:IAO_0000115>
        <oboInOwl:id>GAZ:00148113</oboInOwl:id>
    </rdf:Description>
    <rdf:Description rdf:about="http://purl.obolibrary.org/obo/GAZ_00148114">
        <oboInOwl:hasOBONamespace>GAZ</oboInOwl:hasOBONamespace>
        <obo:IAO_0000115>A tajch.</obo:IAO_0000115>
        <rdfs:label>Richnavske ve&apos;ke jazero</rdfs:label>
        <oboInOwl:id>GAZ:00148114</oboInOwl:id>
    </rdf:Description>
    <rdf:Description rdf:about="http://purl.obolibrary.org/obo/GAZ_00148115">
        <oboInOwl:hasOBONamespace>GAZ</oboInOwl:hasOBONamespace>
        <rdfs:label>Richnavske male jazero</rdfs:label>
        <oboInOwl:id>GAZ:00148115</oboInOwl:id>
        <obo:IAO_0000115>A tajch.</obo:IAO_0000115>
    </rdf:Description>
    <rdf:Description rdf:about="http://purl.obolibrary.org/obo/GAZ_00148117">
        <oboInOwl:id>GAZ:00148117</oboInOwl:id>
        <rdfs:label>Vodarenske male jazero</rdfs:label>
        <obo:IAO_0000115>A tajch.</obo:IAO_0000115>
        <oboInOwl:hasOBONamespace>GAZ</oboInOwl:hasOBONamespace>
    </rdf:Description>
    <rdf:Description rdf:about="http://purl.obolibrary.org/obo/GAZ_00148118">
        <oboInOwl:id>GAZ:00148118</oboInOwl:id>
        <rdfs:label>Vindsachtske dolne jazero</rdfs:label>
        <obo:IAO_0000115>A tajch.</obo:IAO_0000115>
        <oboInOwl:hasOBONamespace>GAZ</oboInOwl:hasOBONamespace>
    </rdf:Description>
    <rdf:Description rdf:about="http://purl.obolibrary.org/obo/GAZ_00148119">
        <obo:IAO_0000115>A tajch.</obo:IAO_0000115>
        <rdfs:label>Vindsachtske horne jazero</rdfs:label>
        <oboInOwl:id>GAZ:00148119</oboInOwl:id>
        <oboInOwl:hasOBONamespace>GAZ</oboInOwl:hasOBONamespace>
    </rdf:Description>
    <rdf:Description rdf:about="http://purl.obolibrary.org/obo/GAZ_00148120">
        <obo:IAO_0000115>A tajch.</obo:IAO_0000115>
        <oboInOwl:id>GAZ:00148120</oboInOwl:id>
        <oboInOwl:hasOBONamespace>GAZ</oboInOwl:hasOBONamespace>
        <rdfs:label>Moderstolnianske jazero</rdfs:label>
    </rdf:Description>
    <rdf:Description rdf:about="http://purl.obolibrary.org/obo/GAZ_00148563">
        <oboInOwl:id>GAZ:00148563</oboInOwl:id>
        <oboInOwl:hasOBONamespace>GAZ</oboInOwl:hasOBONamespace>
        <obo:IAO_0000115>A 316 km long river in Germany (65 km) and the Czech Republic (251 km), left tributary of the Elbe. The source of the river is situated in Bavaria at the foot of Schneeberg mountain in the Fichtelgebirge Range near the town of Weissenstadt. The Ohre flows through the Weissenstadt Lake and the towns Roeslau, Marktleuthen and Hohenberg where it leaves Germany. After approximately 35 km, it crosses the border to Czech Republic to flow through parts of Bohemia. The river passes the cities Cheb, Karlovy Vary, Klasterec nad Ohri, Kadan, Zatec, Louny, and Terezin before flowing into the river Elbe in Litomerice.</obo:IAO_0000115>
        <rdfs:label>Ohre</rdfs:label>
    </rdf:Description>
    <rdf:Description rdf:about="http://purl.obolibrary.org/obo/GAZ_00481281">
        <obo:IAO_0000115>A valley.</obo:IAO_0000115>
        <oboInOwl:id>GAZ:00481281</oboInOwl:id>
        <rdfs:label>Rachkov Zadok</rdfs:label>
        <oboInOwl:hasOBONamespace>GAZ</oboInOwl:hasOBONamespace>
    </rdf:Description>
    <rdf:Description rdf:about="http://purl.obolibrary.org/obo/GAZ_00619830">
        <rdfs:label>Isar-werk Kanal</rdfs:label>
        <obo:IAO_0000115>A river.</obo:IAO_0000115>
        <oboInOwl:id>GAZ:00619830</oboInOwl:id>
        <oboInOwl:hasOBONamespace>GAZ</oboInOwl:hasOBONamespace>
    </rdf:Description>
</rdf:RDF>



<!-- Generated by the OWL API (version 4.5.6) https://github.com/owlcs/owlapi -->

