<?xml version="1.0"?>
<rdf:RDF xmlns="http://purl.obolibrary.org/obo/gaz/subsets/countries/Iceland.owl#"
     xml:base="http://purl.obolibrary.org/obo/gaz/subsets/countries/Iceland.owl"
     xmlns:obo="http://purl.obolibrary.org/obo/"
     xmlns:owl="http://www.w3.org/2002/07/owl#"
     xmlns:rdf="http://www.w3.org/1999/02/22-rdf-syntax-ns#"
     xmlns:xml="http://www.w3.org/XML/1998/namespace"
     xmlns:xsd="http://www.w3.org/2001/XMLSchema#"
     xmlns:rdfs="http://www.w3.org/2000/01/rdf-schema#"
     xmlns:oboInOwl="http://www.geneontology.org/formats/oboInOwl#">
    <owl:Ontology rdf:about="http://purl.obolibrary.org/obo/gaz/subsets/countries/Iceland.owl">
        <owl:imports rdf:resource="http://purl.obolibrary.org/obo/gaz/imports/envo_import.owl"/>
        <owl:imports rdf:resource="http://purl.obolibrary.org/obo/gaz/imports/ro_import.owl"/>
    </owl:Ontology>
    


    <!-- 
    ///////////////////////////////////////////////////////////////////////////////////////
    //
    // Annotation properties
    //
    ///////////////////////////////////////////////////////////////////////////////////////
     -->

    


    <!-- http://purl.obolibrary.org/obo/IAO_0000115 -->

    <owl:AnnotationProperty rdf:about="http://purl.obolibrary.org/obo/IAO_0000115"/>
    


    <!-- http://www.geneontology.org/formats/oboInOwl#hasOBONamespace -->

    <owl:AnnotationProperty rdf:about="http://www.geneontology.org/formats/oboInOwl#hasOBONamespace"/>
    


    <!-- http://www.geneontology.org/formats/oboInOwl#id -->

    <owl:AnnotationProperty rdf:about="http://www.geneontology.org/formats/oboInOwl#id"/>
    


    <!-- 
    ///////////////////////////////////////////////////////////////////////////////////////
    //
    // Object Properties
    //
    ///////////////////////////////////////////////////////////////////////////////////////
     -->

    


    <!-- http://purl.obolibrary.org/obo/RO_0001025 -->

    <owl:ObjectProperty rdf:about="http://purl.obolibrary.org/obo/RO_0001025"/>
    


    <!-- 
    ///////////////////////////////////////////////////////////////////////////////////////
    //
    // Classes
    //
    ///////////////////////////////////////////////////////////////////////////////////////
     -->

    


    <!-- http://purl.obolibrary.org/obo/ENVO_00000009 -->

    <owl:Class rdf:about="http://purl.obolibrary.org/obo/ENVO_00000009"/>
    


    <!-- http://purl.obolibrary.org/obo/ENVO_00000104 -->

    <owl:Class rdf:about="http://purl.obolibrary.org/obo/ENVO_00000104"/>
    


    <!-- http://purl.obolibrary.org/obo/ENVO_00000222 -->

    <owl:Class rdf:about="http://purl.obolibrary.org/obo/ENVO_00000222"/>
    


    <!-- http://purl.obolibrary.org/obo/ENVO_00000305 -->

    <owl:Class rdf:about="http://purl.obolibrary.org/obo/ENVO_00000305"/>
    


    <!-- http://purl.obolibrary.org/obo/ENVO_00000354 -->

    <owl:Class rdf:about="http://purl.obolibrary.org/obo/ENVO_00000354"/>
    


    <!-- http://purl.obolibrary.org/obo/ENVO_00000475 -->

    <owl:Class rdf:about="http://purl.obolibrary.org/obo/ENVO_00000475"/>
    


    <!-- http://purl.obolibrary.org/obo/ENVO_00000856 -->

    <owl:Class rdf:about="http://purl.obolibrary.org/obo/ENVO_00000856"/>
    


    <!-- http://purl.obolibrary.org/obo/GAZ_00001200 -->

    <owl:Class rdf:about="http://purl.obolibrary.org/obo/GAZ_00001200"/>
    


    <!-- http://purl.obolibrary.org/obo/GAZ_00001201 -->

    <owl:Class rdf:about="http://purl.obolibrary.org/obo/GAZ_00001201">
        <rdfs:subClassOf rdf:resource="http://purl.obolibrary.org/obo/GAZ_00001200"/>
    </owl:Class>
    


    <!-- http://purl.obolibrary.org/obo/GAZ_00001202 -->

    <owl:Class rdf:about="http://purl.obolibrary.org/obo/GAZ_00001202">
        <rdfs:subClassOf rdf:resource="http://purl.obolibrary.org/obo/GAZ_00001200"/>
    </owl:Class>
    


    <!-- http://purl.obolibrary.org/obo/GAZ_00001203 -->

    <owl:Class rdf:about="http://purl.obolibrary.org/obo/GAZ_00001203">
        <rdfs:subClassOf rdf:resource="http://purl.obolibrary.org/obo/GAZ_00001200"/>
    </owl:Class>
    


    <!-- http://purl.obolibrary.org/obo/GAZ_00001204 -->

    <owl:Class rdf:about="http://purl.obolibrary.org/obo/GAZ_00001204">
        <rdfs:subClassOf rdf:resource="http://purl.obolibrary.org/obo/GAZ_00001200"/>
    </owl:Class>
    


    <!-- http://purl.obolibrary.org/obo/GAZ_00001205 -->

    <owl:Class rdf:about="http://purl.obolibrary.org/obo/GAZ_00001205">
        <rdfs:subClassOf rdf:resource="http://purl.obolibrary.org/obo/GAZ_00001200"/>
    </owl:Class>
    


    <!-- http://purl.obolibrary.org/obo/GAZ_00001206 -->

    <owl:Class rdf:about="http://purl.obolibrary.org/obo/GAZ_00001206">
        <rdfs:subClassOf rdf:resource="http://purl.obolibrary.org/obo/GAZ_00001200"/>
    </owl:Class>
    


    <!-- http://purl.obolibrary.org/obo/GAZ_00001207 -->

    <owl:Class rdf:about="http://purl.obolibrary.org/obo/GAZ_00001207">
        <rdfs:subClassOf rdf:resource="http://purl.obolibrary.org/obo/GAZ_00001200"/>
    </owl:Class>
    


    <!-- http://purl.obolibrary.org/obo/GAZ_00001208 -->

    <owl:Class rdf:about="http://purl.obolibrary.org/obo/GAZ_00001208">
        <rdfs:subClassOf rdf:resource="http://purl.obolibrary.org/obo/GAZ_00001200"/>
    </owl:Class>
    


    <!-- http://purl.obolibrary.org/obo/GAZ_00007698 -->

    <owl:Class rdf:about="http://purl.obolibrary.org/obo/GAZ_00007698"/>
    


    <!-- http://purl.obolibrary.org/obo/GAZ_00007699 -->

    <owl:Class rdf:about="http://purl.obolibrary.org/obo/GAZ_00007699">
        <rdfs:subClassOf rdf:resource="http://purl.obolibrary.org/obo/GAZ_00007698"/>
    </owl:Class>
    


    <!-- http://purl.obolibrary.org/obo/GAZ_00008737 -->

    <owl:Class rdf:about="http://purl.obolibrary.org/obo/GAZ_00008737">
        <rdfs:subClassOf rdf:resource="http://purl.obolibrary.org/obo/GAZ_00007698"/>
    </owl:Class>
    


    <!-- http://purl.obolibrary.org/obo/GAZ_00008738 -->

    <owl:Class rdf:about="http://purl.obolibrary.org/obo/GAZ_00008738">
        <rdfs:subClassOf rdf:resource="http://purl.obolibrary.org/obo/GAZ_00007698"/>
        <obo:IAO_0000115>A small town in the south of Iceland located 45 km to the east of Reykjavik on Iceland&apos;s main ringroad, Route 1. It is the main town of Hveragerdi municipality. The river Varma runs through the town.</obo:IAO_0000115>
        <oboInOwl:hasOBONamespace>GAZ</oboInOwl:hasOBONamespace>
        <oboInOwl:id>GAZ:00008738</oboInOwl:id>
        <rdfs:label>Hveragerdi</rdfs:label>
    </owl:Class>
    


    <!-- http://purl.obolibrary.org/obo/GAZ_00280387 -->

    <owl:Class rdf:about="http://purl.obolibrary.org/obo/GAZ_00280387"/>
    


    <!-- http://purl.obolibrary.org/obo/GAZ_00280388 -->

    <owl:Class rdf:about="http://purl.obolibrary.org/obo/GAZ_00280388">
        <rdfs:subClassOf rdf:resource="http://purl.obolibrary.org/obo/GAZ_00280387"/>
        <obo:IAO_0000115>A lava cave and pseudocrater. Sie liegt in der Nahe des Weges der Thingvellir und Laugarvatn verbindet.</obo:IAO_0000115>
        <oboInOwl:hasOBONamespace>GAZ</oboInOwl:hasOBONamespace>
        <oboInOwl:id>GAZ:00280388</oboInOwl:id>
        <rdfs:label>Tintron</rdfs:label>
    </owl:Class>
    


    <!-- 
    ///////////////////////////////////////////////////////////////////////////////////////
    //
    // Individuals
    //
    ///////////////////////////////////////////////////////////////////////////////////////
     -->

    


    <!-- http://purl.obolibrary.org/obo/GAZ_00000843 -->

    <owl:NamedIndividual rdf:about="http://purl.obolibrary.org/obo/GAZ_00000843">
        <rdf:type rdf:resource="http://purl.obolibrary.org/obo/ENVO_00000009"/>
        <obo:IAO_0000115>A country in northern Europe, comprising the island of Iceland and its outlying islands in the North Atlantic Ocean between the rest of Europe and Greenland.</obo:IAO_0000115>
        <oboInOwl:hasOBONamespace>GAZ</oboInOwl:hasOBONamespace>
        <oboInOwl:id>GAZ:00000843</oboInOwl:id>
        <rdfs:label>Iceland</rdfs:label>
    </owl:NamedIndividual>
    


    <!-- http://purl.obolibrary.org/obo/GAZ_00001200 -->

    <owl:NamedIndividual rdf:about="http://purl.obolibrary.org/obo/GAZ_00001200">
        <obo:RO_0001025 rdf:resource="http://purl.obolibrary.org/obo/GAZ_00000843"/>
    </owl:NamedIndividual>
    


    <!-- http://purl.obolibrary.org/obo/GAZ_00001201 -->

    <owl:NamedIndividual rdf:about="http://purl.obolibrary.org/obo/GAZ_00001201"/>
    


    <!-- http://purl.obolibrary.org/obo/GAZ_00001202 -->

    <owl:NamedIndividual rdf:about="http://purl.obolibrary.org/obo/GAZ_00001202"/>
    


    <!-- http://purl.obolibrary.org/obo/GAZ_00001203 -->

    <owl:NamedIndividual rdf:about="http://purl.obolibrary.org/obo/GAZ_00001203"/>
    


    <!-- http://purl.obolibrary.org/obo/GAZ_00001204 -->

    <owl:NamedIndividual rdf:about="http://purl.obolibrary.org/obo/GAZ_00001204"/>
    


    <!-- http://purl.obolibrary.org/obo/GAZ_00001205 -->

    <owl:NamedIndividual rdf:about="http://purl.obolibrary.org/obo/GAZ_00001205"/>
    


    <!-- http://purl.obolibrary.org/obo/GAZ_00001206 -->

    <owl:NamedIndividual rdf:about="http://purl.obolibrary.org/obo/GAZ_00001206"/>
    


    <!-- http://purl.obolibrary.org/obo/GAZ_00001207 -->

    <owl:NamedIndividual rdf:about="http://purl.obolibrary.org/obo/GAZ_00001207"/>
    


    <!-- http://purl.obolibrary.org/obo/GAZ_00001208 -->

    <owl:NamedIndividual rdf:about="http://purl.obolibrary.org/obo/GAZ_00001208"/>
    


    <!-- http://purl.obolibrary.org/obo/GAZ_00001210 -->

    <owl:NamedIndividual rdf:about="http://purl.obolibrary.org/obo/GAZ_00001210">
        <obo:RO_0001025 rdf:resource="http://purl.obolibrary.org/obo/GAZ_00001207"/>
        <obo:RO_0001025 rdf:resource="http://purl.obolibrary.org/obo/GAZ_00053339"/>
        <obo:IAO_0000115>An island in Skjalfandi bay located about 8.7 km from Husavik, in northern Iceland.</obo:IAO_0000115>
        <oboInOwl:hasOBONamespace>GAZ</oboInOwl:hasOBONamespace>
        <oboInOwl:id>GAZ:00001210</oboInOwl:id>
        <rdfs:label>Flatey [NE]</rdfs:label>
    </owl:NamedIndividual>
    


    <!-- http://purl.obolibrary.org/obo/GAZ_00001211 -->

    <owl:NamedIndividual rdf:about="http://purl.obolibrary.org/obo/GAZ_00001211">
        <obo:RO_0001025 rdf:resource="http://purl.obolibrary.org/obo/GAZ_00053332"/>
        <obo:IAO_0000115>An island in Skagafjoerdur in Iceland. The island is the remnant of a 700,000 year old volcano, mostly made of volcanic tuff, forming a massive rock fortress.</obo:IAO_0000115>
        <oboInOwl:hasOBONamespace>GAZ</oboInOwl:hasOBONamespace>
        <oboInOwl:id>GAZ:00001211</oboInOwl:id>
        <rdfs:label>Drangey</rdfs:label>
    </owl:NamedIndividual>
    


    <!-- http://purl.obolibrary.org/obo/GAZ_00001212 -->

    <owl:NamedIndividual rdf:about="http://purl.obolibrary.org/obo/GAZ_00001212">
        <obo:RO_0001025 rdf:resource="http://purl.obolibrary.org/obo/GAZ_00053333"/>
        <obo:IAO_0000115>An island in Breidafjoerdur. It consists of the main island and forty other smaller islands.</obo:IAO_0000115>
        <oboInOwl:hasOBONamespace>GAZ</oboInOwl:hasOBONamespace>
        <oboInOwl:id>GAZ:00001212</oboInOwl:id>
        <rdfs:label>Flatey</rdfs:label>
    </owl:NamedIndividual>
    


    <!-- http://purl.obolibrary.org/obo/GAZ_00001213 -->

    <owl:NamedIndividual rdf:about="http://purl.obolibrary.org/obo/GAZ_00001213">
        <obo:RO_0001025 rdf:resource="http://purl.obolibrary.org/obo/GAZ_00020010"/>
        <obo:RO_0001025 rdf:resource="http://purl.obolibrary.org/obo/GAZ_00280522"/>
        <obo:IAO_0000115>A small island 40 km north of Iceland, situated directly on the Arctic Circle, with the highest elevation of 105 m.</obo:IAO_0000115>
        <oboInOwl:hasOBONamespace>GAZ</oboInOwl:hasOBONamespace>
        <oboInOwl:id>GAZ:00001213</oboInOwl:id>
        <rdfs:label>Grimsey [NE]</rdfs:label>
    </owl:NamedIndividual>
    


    <!-- http://purl.obolibrary.org/obo/GAZ_00001214 -->

    <owl:NamedIndividual rdf:about="http://purl.obolibrary.org/obo/GAZ_00001214">
        <obo:RO_0001025 rdf:resource="http://purl.obolibrary.org/obo/GAZ_00001201"/>
        <obo:RO_0001025 rdf:resource="http://purl.obolibrary.org/obo/GAZ_00280523"/>
        <obo:IAO_0000115>A small island about 10 miles off the coast of the Reykjanes Peninsula, southwest Iceland.</obo:IAO_0000115>
        <oboInOwl:hasOBONamespace>GAZ</oboInOwl:hasOBONamespace>
        <oboInOwl:id>GAZ:00001214</oboInOwl:id>
        <rdfs:label>Eldey</rdfs:label>
    </owl:NamedIndividual>
    


    <!-- http://purl.obolibrary.org/obo/GAZ_00001215 -->

    <owl:NamedIndividual rdf:about="http://purl.obolibrary.org/obo/GAZ_00001215">
        <obo:RO_0001025 rdf:resource="http://purl.obolibrary.org/obo/GAZ_00280134"/>
        <obo:IAO_0000115>An island.</obo:IAO_0000115>
        <oboInOwl:hasOBONamespace>GAZ</oboInOwl:hasOBONamespace>
        <oboInOwl:id>GAZ:00001215</oboInOwl:id>
        <rdfs:label>Engey</rdfs:label>
    </owl:NamedIndividual>
    


    <!-- http://purl.obolibrary.org/obo/GAZ_00001216 -->

    <owl:NamedIndividual rdf:about="http://purl.obolibrary.org/obo/GAZ_00001216">
        <obo:RO_0001025 rdf:resource="http://purl.obolibrary.org/obo/GAZ_00008739"/>
        <obo:IAO_0000115>The largest island (13.4 km2) in the Vestmannaeyjar cluster, approximately 7.4 km off the south coast of Iceland.</obo:IAO_0000115>
        <oboInOwl:hasOBONamespace>GAZ</oboInOwl:hasOBONamespace>
        <oboInOwl:id>GAZ:00001216</oboInOwl:id>
        <rdfs:label>Heimaey</rdfs:label>
    </owl:NamedIndividual>
    


    <!-- http://purl.obolibrary.org/obo/GAZ_00001217 -->

    <owl:NamedIndividual rdf:about="http://purl.obolibrary.org/obo/GAZ_00001217">
        <obo:RO_0001025 rdf:resource="http://purl.obolibrary.org/obo/GAZ_00280134"/>
        <obo:IAO_0000115>The largest island of the Kollafjoerdur Bay in Iceland, near the capital of Reykjavik.</obo:IAO_0000115>
        <oboInOwl:hasOBONamespace>GAZ</oboInOwl:hasOBONamespace>
        <oboInOwl:id>GAZ:00001217</oboInOwl:id>
        <rdfs:label>Videy</rdfs:label>
    </owl:NamedIndividual>
    


    <!-- http://purl.obolibrary.org/obo/GAZ_00001218 -->

    <owl:NamedIndividual rdf:about="http://purl.obolibrary.org/obo/GAZ_00001218">
        <obo:RO_0001025 rdf:resource="http://purl.obolibrary.org/obo/GAZ_00020010"/>
        <obo:RO_0001025 rdf:resource="http://purl.obolibrary.org/obo/GAZ_00053354"/>
        <obo:IAO_0000115>A small island off the north coast of Iceland, situated approximately 35 km north of Akureyri.</obo:IAO_0000115>
        <oboInOwl:hasOBONamespace>GAZ</oboInOwl:hasOBONamespace>
        <oboInOwl:id>GAZ:00001218</oboInOwl:id>
        <rdfs:label>Hrisey</rdfs:label>
    </owl:NamedIndividual>
    


    <!-- http://purl.obolibrary.org/obo/GAZ_00001219 -->

    <owl:NamedIndividual rdf:about="http://purl.obolibrary.org/obo/GAZ_00001219">
        <obo:RO_0001025 rdf:resource="http://purl.obolibrary.org/obo/GAZ_00280522"/>
        <obo:IAO_0000115>A tiny island 105 km off the northern coast of Iceland, 74 km North-Northwest of the island of Grimsey.</obo:IAO_0000115>
        <oboInOwl:hasOBONamespace>GAZ</oboInOwl:hasOBONamespace>
        <oboInOwl:id>GAZ:00001219</oboInOwl:id>
        <rdfs:label>Kolbeinsey</rdfs:label>
    </owl:NamedIndividual>
    


    <!-- http://purl.obolibrary.org/obo/GAZ_00001220 -->

    <owl:NamedIndividual rdf:about="http://purl.obolibrary.org/obo/GAZ_00001220">
        <obo:RO_0001025 rdf:resource="http://purl.obolibrary.org/obo/GAZ_00020003"/>
        <obo:RO_0001025 rdf:resource="http://purl.obolibrary.org/obo/GAZ_00280523"/>
        <obo:IAO_0000115>An island off the south east of Iceland.</obo:IAO_0000115>
        <oboInOwl:hasOBONamespace>GAZ</oboInOwl:hasOBONamespace>
        <oboInOwl:id>GAZ:00001220</oboInOwl:id>
        <rdfs:label>Papey</rdfs:label>
    </owl:NamedIndividual>
    


    <!-- http://purl.obolibrary.org/obo/GAZ_00001221 -->

    <owl:NamedIndividual rdf:about="http://purl.obolibrary.org/obo/GAZ_00001221">
        <obo:RO_0001025 rdf:resource="http://purl.obolibrary.org/obo/GAZ_00053332"/>
        <obo:IAO_0000115>An island in the Skagafjoerdur.</obo:IAO_0000115>
        <oboInOwl:hasOBONamespace>GAZ</oboInOwl:hasOBONamespace>
        <oboInOwl:id>GAZ:00001221</oboInOwl:id>
        <rdfs:label>Malmey</rdfs:label>
    </owl:NamedIndividual>
    


    <!-- http://purl.obolibrary.org/obo/GAZ_00001222 -->

    <owl:NamedIndividual rdf:about="http://purl.obolibrary.org/obo/GAZ_00001222">
        <obo:RO_0001025 rdf:resource="http://purl.obolibrary.org/obo/GAZ_00145755"/>
        <obo:IAO_0000115>An island.</obo:IAO_0000115>
        <oboInOwl:hasOBONamespace>GAZ</oboInOwl:hasOBONamespace>
        <oboInOwl:id>GAZ:00001222</oboInOwl:id>
        <rdfs:label>Aedey</rdfs:label>
    </owl:NamedIndividual>
    


    <!-- http://purl.obolibrary.org/obo/GAZ_00001223 -->

    <owl:NamedIndividual rdf:about="http://purl.obolibrary.org/obo/GAZ_00001223">
        <rdf:type rdf:resource="http://purl.obolibrary.org/obo/ENVO_00000222"/>
        <obo:RO_0001025 rdf:resource="http://purl.obolibrary.org/obo/GAZ_00008739"/>
        <obo:IAO_0000115>A volcanic island off the southern coast of Iceland. At 63.18degN 20.36degW it is also the southernmost point of Iceland. It was formed in a volcanic eruption which began 130 m below sea level, and reached the surface on 1963-11-14.</obo:IAO_0000115>
        <oboInOwl:hasOBONamespace>GAZ</oboInOwl:hasOBONamespace>
        <oboInOwl:id>GAZ:00001223</oboInOwl:id>
        <rdfs:label>Surtsey</rdfs:label>
    </owl:NamedIndividual>
    


    <!-- http://purl.obolibrary.org/obo/GAZ_00001224 -->

    <owl:NamedIndividual rdf:about="http://purl.obolibrary.org/obo/GAZ_00001224">
        <obo:RO_0001025 rdf:resource="http://purl.obolibrary.org/obo/GAZ_00280523"/>
        <obo:IAO_0000115>An island off the E coast of Iceland.</obo:IAO_0000115>
        <oboInOwl:hasOBONamespace>GAZ</oboInOwl:hasOBONamespace>
        <oboInOwl:id>GAZ:00001224</oboInOwl:id>
        <rdfs:label>Hvalbakur</rdfs:label>
    </owl:NamedIndividual>
    


    <!-- http://purl.obolibrary.org/obo/GAZ_00001225 -->

    <owl:NamedIndividual rdf:about="http://purl.obolibrary.org/obo/GAZ_00001225">
        <obo:RO_0001025 rdf:resource="http://purl.obolibrary.org/obo/GAZ_00001203"/>
        <obo:RO_0001025 rdf:resource="http://purl.obolibrary.org/obo/GAZ_00280523"/>
        <obo:IAO_0000115>An island.</obo:IAO_0000115>
        <oboInOwl:hasOBONamespace>GAZ</oboInOwl:hasOBONamespace>
        <oboInOwl:id>GAZ:00001225</oboInOwl:id>
        <rdfs:label>Vigur [East]</rdfs:label>
    </owl:NamedIndividual>
    


    <!-- http://purl.obolibrary.org/obo/GAZ_00007698 -->

    <owl:NamedIndividual rdf:about="http://purl.obolibrary.org/obo/GAZ_00007698">
        <obo:RO_0001025 rdf:resource="http://purl.obolibrary.org/obo/GAZ_00000843"/>
    </owl:NamedIndividual>
    


    <!-- http://purl.obolibrary.org/obo/GAZ_00007699 -->

    <owl:NamedIndividual rdf:about="http://purl.obolibrary.org/obo/GAZ_00007699">
        <obo:RO_0001025 rdf:resource="http://purl.obolibrary.org/obo/GAZ_02000605"/>
    </owl:NamedIndividual>
    


    <!-- http://purl.obolibrary.org/obo/GAZ_00007720 -->

    <owl:NamedIndividual rdf:about="http://purl.obolibrary.org/obo/GAZ_00007720">
        <obo:RO_0001025 rdf:resource="http://purl.obolibrary.org/obo/GAZ_00280276"/>
        <obo:IAO_0000115>A geyser. Located in the Haukadalur valley, Iceland.</obo:IAO_0000115>
        <oboInOwl:hasOBONamespace>GAZ</oboInOwl:hasOBONamespace>
        <oboInOwl:id>GAZ:00007720</oboInOwl:id>
        <rdfs:label>Geysir</rdfs:label>
    </owl:NamedIndividual>
    


    <!-- http://purl.obolibrary.org/obo/GAZ_00007721 -->

    <owl:NamedIndividual rdf:about="http://purl.obolibrary.org/obo/GAZ_00007721">
        <obo:RO_0001025 rdf:resource="http://purl.obolibrary.org/obo/GAZ_00001204"/>
        <obo:IAO_0000115>A populated place.</obo:IAO_0000115>
        <oboInOwl:hasOBONamespace>GAZ</oboInOwl:hasOBONamespace>
        <oboInOwl:id>GAZ:00007721</oboInOwl:id>
        <rdfs:label>Hruni</rdfs:label>
    </owl:NamedIndividual>
    


    <!-- http://purl.obolibrary.org/obo/GAZ_00008175 -->

    <owl:NamedIndividual rdf:about="http://purl.obolibrary.org/obo/GAZ_00008175">
        <obo:RO_0001025 rdf:resource="http://purl.obolibrary.org/obo/GAZ_00001201"/>
        <obo:IAO_0000115>A peninsula at the south-western end of Iceland, near the capital of Reykjavik.</obo:IAO_0000115>
        <oboInOwl:hasOBONamespace>GAZ</oboInOwl:hasOBONamespace>
        <oboInOwl:id>GAZ:00008175</oboInOwl:id>
        <rdfs:label>Reykjanes Peninsula</rdfs:label>
    </owl:NamedIndividual>
    


    <!-- http://purl.obolibrary.org/obo/GAZ_00008736 -->

    <owl:NamedIndividual rdf:about="http://purl.obolibrary.org/obo/GAZ_00008736">
        <obo:RO_0001025 rdf:resource="http://purl.obolibrary.org/obo/GAZ_00008175"/>
        <obo:IAO_0000115>The geothermal area Krysuvik is situated on the Reykjanes peninsula in Iceland. It is in the south of Reykjanes in the middle of the fissure zone on the Mid-Atlantic Ridge which traverses Iceland diagonally from the south-west to the north-east of the island.</obo:IAO_0000115>
        <oboInOwl:hasOBONamespace>GAZ</oboInOwl:hasOBONamespace>
        <oboInOwl:id>GAZ:00008736</oboInOwl:id>
        <rdfs:label>Krysuvik</rdfs:label>
    </owl:NamedIndividual>
    


    <!-- http://purl.obolibrary.org/obo/GAZ_00008737 -->

    <owl:NamedIndividual rdf:about="http://purl.obolibrary.org/obo/GAZ_00008737">
        <obo:RO_0001025 rdf:resource="http://purl.obolibrary.org/obo/GAZ_02000603"/>
    </owl:NamedIndividual>
    


    <!-- http://purl.obolibrary.org/obo/GAZ_00008739 -->

    <owl:NamedIndividual rdf:about="http://purl.obolibrary.org/obo/GAZ_00008739">
        <obo:RO_0001025 rdf:resource="http://purl.obolibrary.org/obo/GAZ_00280523"/>
        <obo:RO_0001025 rdf:resource="http://purl.obolibrary.org/obo/GAZ_02000604"/>
        <obo:IAO_0000115>A small archipelago off the south coast of Iceland.</obo:IAO_0000115>
        <oboInOwl:hasOBONamespace>GAZ</oboInOwl:hasOBONamespace>
        <oboInOwl:id>GAZ:00008739</oboInOwl:id>
        <rdfs:label>Vestmannaeyjar</rdfs:label>
    </owl:NamedIndividual>
    


    <!-- http://purl.obolibrary.org/obo/GAZ_00019994 -->

    <owl:NamedIndividual rdf:about="http://purl.obolibrary.org/obo/GAZ_00019994">
        <rdf:type rdf:resource="http://purl.obolibrary.org/obo/ENVO_00000856"/>
        <obo:RO_0001025 rdf:resource="http://purl.obolibrary.org/obo/GAZ_00001208"/>
        <obo:IAO_0000115>A municipality in the Greater Reykjavik area of Iceland.</obo:IAO_0000115>
        <oboInOwl:hasOBONamespace>GAZ</oboInOwl:hasOBONamespace>
        <oboInOwl:id>GAZ:00019994</oboInOwl:id>
        <rdfs:label>Municipality of Gardabaer</rdfs:label>
    </owl:NamedIndividual>
    


    <!-- http://purl.obolibrary.org/obo/GAZ_00019995 -->

    <owl:NamedIndividual rdf:about="http://purl.obolibrary.org/obo/GAZ_00019995">
        <rdf:type rdf:resource="http://purl.obolibrary.org/obo/ENVO_00000856"/>
        <obo:RO_0001025 rdf:resource="http://purl.obolibrary.org/obo/GAZ_00001208"/>
        <obo:IAO_0000115>A municipality.</obo:IAO_0000115>
        <oboInOwl:hasOBONamespace>GAZ</oboInOwl:hasOBONamespace>
        <oboInOwl:id>GAZ:00019995</oboInOwl:id>
        <rdfs:label>Municipality of Hafnarfjardarkaupstadur</rdfs:label>
    </owl:NamedIndividual>
    


    <!-- http://purl.obolibrary.org/obo/GAZ_00019996 -->

    <owl:NamedIndividual rdf:about="http://purl.obolibrary.org/obo/GAZ_00019996">
        <rdf:type rdf:resource="http://purl.obolibrary.org/obo/ENVO_00000856"/>
        <obo:RO_0001025 rdf:resource="http://purl.obolibrary.org/obo/GAZ_00001208"/>
        <obo:IAO_0000115>A municipality.</obo:IAO_0000115>
        <oboInOwl:hasOBONamespace>GAZ</oboInOwl:hasOBONamespace>
        <oboInOwl:id>GAZ:00019996</oboInOwl:id>
        <rdfs:label>Municipality of Kjosarhreppur</rdfs:label>
    </owl:NamedIndividual>
    


    <!-- http://purl.obolibrary.org/obo/GAZ_00019997 -->

    <owl:NamedIndividual rdf:about="http://purl.obolibrary.org/obo/GAZ_00019997">
        <rdf:type rdf:resource="http://purl.obolibrary.org/obo/ENVO_00000856"/>
        <obo:RO_0001025 rdf:resource="http://purl.obolibrary.org/obo/GAZ_00001208"/>
        <obo:IAO_0000115>A municipality. Located immediately south of Reykjavik and is part of the Greater Reykjavik Area.</obo:IAO_0000115>
        <oboInOwl:hasOBONamespace>GAZ</oboInOwl:hasOBONamespace>
        <oboInOwl:id>GAZ:00019997</oboInOwl:id>
        <rdfs:label>Municipality of Kopavogsbaer</rdfs:label>
    </owl:NamedIndividual>
    


    <!-- http://purl.obolibrary.org/obo/GAZ_00019998 -->

    <owl:NamedIndividual rdf:about="http://purl.obolibrary.org/obo/GAZ_00019998">
        <rdf:type rdf:resource="http://purl.obolibrary.org/obo/ENVO_00000856"/>
        <obo:RO_0001025 rdf:resource="http://purl.obolibrary.org/obo/GAZ_00001208"/>
        <obo:IAO_0000115>A municipality. Located in south-west Iceland, situated some 17 km north of the country&apos;s capital, Reykjavik.</obo:IAO_0000115>
        <oboInOwl:hasOBONamespace>GAZ</oboInOwl:hasOBONamespace>
        <oboInOwl:id>GAZ:00019998</oboInOwl:id>
        <rdfs:label>Municipality of Mosfellsbaer</rdfs:label>
    </owl:NamedIndividual>
    


    <!-- http://purl.obolibrary.org/obo/GAZ_00019999 -->

    <owl:NamedIndividual rdf:about="http://purl.obolibrary.org/obo/GAZ_00019999">
        <rdf:type rdf:resource="http://purl.obolibrary.org/obo/ENVO_00000856"/>
        <obo:RO_0001025 rdf:resource="http://purl.obolibrary.org/obo/GAZ_00001208"/>
        <obo:IAO_0000115>A municipality. Located within the Greater Reykjavik area.</obo:IAO_0000115>
        <oboInOwl:hasOBONamespace>GAZ</oboInOwl:hasOBONamespace>
        <oboInOwl:id>GAZ:00019999</oboInOwl:id>
        <rdfs:label>Municipality of Seltjarnarneskaupstadur</rdfs:label>
    </owl:NamedIndividual>
    


    <!-- http://purl.obolibrary.org/obo/GAZ_00020000 -->

    <owl:NamedIndividual rdf:about="http://purl.obolibrary.org/obo/GAZ_00020000">
        <obo:RO_0001025 rdf:resource="http://purl.obolibrary.org/obo/GAZ_00001208"/>
        <obo:IAO_0000115>A municipallity.</obo:IAO_0000115>
        <oboInOwl:hasOBONamespace>GAZ</oboInOwl:hasOBONamespace>
        <oboInOwl:id>GAZ:00020000</oboInOwl:id>
        <rdfs:label>Municipality of Alftanes</rdfs:label>
    </owl:NamedIndividual>
    


    <!-- http://purl.obolibrary.org/obo/GAZ_00020001 -->

    <owl:NamedIndividual rdf:about="http://purl.obolibrary.org/obo/GAZ_00020001">
        <rdf:type rdf:resource="http://purl.obolibrary.org/obo/ENVO_00000856"/>
        <obo:RO_0001025 rdf:resource="http://purl.obolibrary.org/obo/GAZ_00001203"/>
        <obo:IAO_0000115>A municipality.</obo:IAO_0000115>
        <oboInOwl:hasOBONamespace>GAZ</oboInOwl:hasOBONamespace>
        <oboInOwl:id>GAZ:00020001</oboInOwl:id>
        <rdfs:label>Borgarfjardarhreppur</rdfs:label>
    </owl:NamedIndividual>
    


    <!-- http://purl.obolibrary.org/obo/GAZ_00020002 -->

    <owl:NamedIndividual rdf:about="http://purl.obolibrary.org/obo/GAZ_00020002">
        <rdf:type rdf:resource="http://purl.obolibrary.org/obo/ENVO_00000856"/>
        <obo:RO_0001025 rdf:resource="http://purl.obolibrary.org/obo/GAZ_00001203"/>
        <obo:IAO_0000115>A municipality.</obo:IAO_0000115>
        <oboInOwl:hasOBONamespace>GAZ</oboInOwl:hasOBONamespace>
        <oboInOwl:id>GAZ:00020002</oboInOwl:id>
        <rdfs:label>Breiddalshreppur</rdfs:label>
    </owl:NamedIndividual>
    


    <!-- http://purl.obolibrary.org/obo/GAZ_00020003 -->

    <owl:NamedIndividual rdf:about="http://purl.obolibrary.org/obo/GAZ_00020003">
        <rdf:type rdf:resource="http://purl.obolibrary.org/obo/ENVO_00000856"/>
        <obo:RO_0001025 rdf:resource="http://purl.obolibrary.org/obo/GAZ_00001203"/>
        <obo:IAO_0000115>A municipality.</obo:IAO_0000115>
        <oboInOwl:hasOBONamespace>GAZ</oboInOwl:hasOBONamespace>
        <oboInOwl:id>GAZ:00020003</oboInOwl:id>
        <rdfs:label>Djupavogshreppur</rdfs:label>
    </owl:NamedIndividual>
    


    <!-- http://purl.obolibrary.org/obo/GAZ_00020004 -->

    <owl:NamedIndividual rdf:about="http://purl.obolibrary.org/obo/GAZ_00020004">
        <rdf:type rdf:resource="http://purl.obolibrary.org/obo/ENVO_00000856"/>
        <obo:RO_0001025 rdf:resource="http://purl.obolibrary.org/obo/GAZ_00001203"/>
        <obo:IAO_0000115>A municipality.</obo:IAO_0000115>
        <oboInOwl:hasOBONamespace>GAZ</oboInOwl:hasOBONamespace>
        <oboInOwl:id>GAZ:00020004</oboInOwl:id>
        <rdfs:label>Municipality of Fjardabyggd</rdfs:label>
    </owl:NamedIndividual>
    


    <!-- http://purl.obolibrary.org/obo/GAZ_00020005 -->

    <owl:NamedIndividual rdf:about="http://purl.obolibrary.org/obo/GAZ_00020005">
        <rdf:type rdf:resource="http://purl.obolibrary.org/obo/ENVO_00000856"/>
        <obo:RO_0001025 rdf:resource="http://purl.obolibrary.org/obo/GAZ_00001203"/>
        <obo:IAO_0000115>A municipality.</obo:IAO_0000115>
        <oboInOwl:hasOBONamespace>GAZ</oboInOwl:hasOBONamespace>
        <oboInOwl:id>GAZ:00020005</oboInOwl:id>
        <rdfs:label>Sveitarfelagid Fljotsdalsherad</rdfs:label>
    </owl:NamedIndividual>
    


    <!-- http://purl.obolibrary.org/obo/GAZ_00020006 -->

    <owl:NamedIndividual rdf:about="http://purl.obolibrary.org/obo/GAZ_00020006">
        <rdf:type rdf:resource="http://purl.obolibrary.org/obo/ENVO_00000856"/>
        <obo:RO_0001025 rdf:resource="http://purl.obolibrary.org/obo/GAZ_00001203"/>
        <obo:IAO_0000115>A municipality.</obo:IAO_0000115>
        <oboInOwl:hasOBONamespace>GAZ</oboInOwl:hasOBONamespace>
        <oboInOwl:id>GAZ:00020006</oboInOwl:id>
        <rdfs:label>Fljotsdalshreppur</rdfs:label>
    </owl:NamedIndividual>
    


    <!-- http://purl.obolibrary.org/obo/GAZ_00020007 -->

    <owl:NamedIndividual rdf:about="http://purl.obolibrary.org/obo/GAZ_00020007">
        <rdf:type rdf:resource="http://purl.obolibrary.org/obo/ENVO_00000856"/>
        <obo:RO_0001025 rdf:resource="http://purl.obolibrary.org/obo/GAZ_00001203"/>
        <obo:IAO_0000115>A municipality.</obo:IAO_0000115>
        <oboInOwl:hasOBONamespace>GAZ</oboInOwl:hasOBONamespace>
        <oboInOwl:id>GAZ:00020007</oboInOwl:id>
        <rdfs:label>Municipality of Seydisfjardarkaupstadur</rdfs:label>
    </owl:NamedIndividual>
    


    <!-- http://purl.obolibrary.org/obo/GAZ_00020008 -->

    <owl:NamedIndividual rdf:about="http://purl.obolibrary.org/obo/GAZ_00020008">
        <rdf:type rdf:resource="http://purl.obolibrary.org/obo/ENVO_00000856"/>
        <obo:RO_0001025 rdf:resource="http://purl.obolibrary.org/obo/GAZ_00001203"/>
        <obo:IAO_0000115>A municipality.</obo:IAO_0000115>
        <oboInOwl:hasOBONamespace>GAZ</oboInOwl:hasOBONamespace>
        <oboInOwl:id>GAZ:00020008</oboInOwl:id>
        <rdfs:label>Sveitarfelagid Hornafjoerdur</rdfs:label>
    </owl:NamedIndividual>
    


    <!-- http://purl.obolibrary.org/obo/GAZ_00020009 -->

    <owl:NamedIndividual rdf:about="http://purl.obolibrary.org/obo/GAZ_00020009">
        <rdf:type rdf:resource="http://purl.obolibrary.org/obo/ENVO_00000856"/>
        <obo:RO_0001025 rdf:resource="http://purl.obolibrary.org/obo/GAZ_00001203"/>
        <obo:IAO_0000115>A municipality.</obo:IAO_0000115>
        <oboInOwl:hasOBONamespace>GAZ</oboInOwl:hasOBONamespace>
        <oboInOwl:id>GAZ:00020009</oboInOwl:id>
        <rdfs:label>Vopnafjardsarhreppur</rdfs:label>
    </owl:NamedIndividual>
    


    <!-- http://purl.obolibrary.org/obo/GAZ_00020010 -->

    <owl:NamedIndividual rdf:about="http://purl.obolibrary.org/obo/GAZ_00020010">
        <rdf:type rdf:resource="http://purl.obolibrary.org/obo/ENVO_00000856"/>
        <obo:RO_0001025 rdf:resource="http://purl.obolibrary.org/obo/GAZ_00001207"/>
        <obo:IAO_0000115>A municipality.</obo:IAO_0000115>
        <oboInOwl:hasOBONamespace>GAZ</oboInOwl:hasOBONamespace>
        <oboInOwl:id>GAZ:00020010</oboInOwl:id>
        <rdfs:label>Municipality of Akureyrarkaupstadur</rdfs:label>
    </owl:NamedIndividual>
    


    <!-- http://purl.obolibrary.org/obo/GAZ_00020011 -->

    <owl:NamedIndividual rdf:about="http://purl.obolibrary.org/obo/GAZ_00020011">
        <rdf:type rdf:resource="http://purl.obolibrary.org/obo/ENVO_00000856"/>
        <obo:RO_0001025 rdf:resource="http://purl.obolibrary.org/obo/GAZ_00001207"/>
        <obo:IAO_0000115>A municipality.</obo:IAO_0000115>
        <oboInOwl:hasOBONamespace>GAZ</oboInOwl:hasOBONamespace>
        <oboInOwl:id>GAZ:00020011</oboInOwl:id>
        <rdfs:label>Arnarneshreppur</rdfs:label>
    </owl:NamedIndividual>
    


    <!-- http://purl.obolibrary.org/obo/GAZ_00020012 -->

    <owl:NamedIndividual rdf:about="http://purl.obolibrary.org/obo/GAZ_00020012">
        <obo:RO_0001025 rdf:resource="http://purl.obolibrary.org/obo/GAZ_00001207"/>
        <obo:IAO_0000115>A municipaluty.</obo:IAO_0000115>
        <oboInOwl:hasOBONamespace>GAZ</oboInOwl:hasOBONamespace>
        <oboInOwl:id>GAZ:00020012</oboInOwl:id>
        <rdfs:label>Municipality of Dalvikurbyggd</rdfs:label>
    </owl:NamedIndividual>
    


    <!-- http://purl.obolibrary.org/obo/GAZ_00020013 -->

    <owl:NamedIndividual rdf:about="http://purl.obolibrary.org/obo/GAZ_00020013">
        <rdf:type rdf:resource="http://purl.obolibrary.org/obo/ENVO_00000856"/>
        <obo:RO_0001025 rdf:resource="http://purl.obolibrary.org/obo/GAZ_00001207"/>
        <obo:IAO_0000115>A municipality.</obo:IAO_0000115>
        <oboInOwl:hasOBONamespace>GAZ</oboInOwl:hasOBONamespace>
        <oboInOwl:id>GAZ:00020013</oboInOwl:id>
        <rdfs:label>Municipality of Eyjafjardarsveit</rdfs:label>
    </owl:NamedIndividual>
    


    <!-- http://purl.obolibrary.org/obo/GAZ_00020014 -->

    <owl:NamedIndividual rdf:about="http://purl.obolibrary.org/obo/GAZ_00020014">
        <rdf:type rdf:resource="http://purl.obolibrary.org/obo/ENVO_00000856"/>
        <obo:RO_0001025 rdf:resource="http://purl.obolibrary.org/obo/GAZ_00001207"/>
        <obo:IAO_0000115>A municipality.</obo:IAO_0000115>
        <oboInOwl:hasOBONamespace>GAZ</oboInOwl:hasOBONamespace>
        <oboInOwl:id>GAZ:00020014</oboInOwl:id>
        <rdfs:label>Municipality of Fjallabyggd</rdfs:label>
    </owl:NamedIndividual>
    


    <!-- http://purl.obolibrary.org/obo/GAZ_00020015 -->

    <owl:NamedIndividual rdf:about="http://purl.obolibrary.org/obo/GAZ_00020015">
        <rdf:type rdf:resource="http://purl.obolibrary.org/obo/ENVO_00000856"/>
        <obo:RO_0001025 rdf:resource="http://purl.obolibrary.org/obo/GAZ_00001213"/>
        <obo:IAO_0000115>A former municipality. Merged 2009-05-31.</obo:IAO_0000115>
        <oboInOwl:hasOBONamespace>GAZ</oboInOwl:hasOBONamespace>
        <oboInOwl:id>GAZ:00020015</oboInOwl:id>
        <rdfs:label>[Former] Grimseyjarhreppur</rdfs:label>
    </owl:NamedIndividual>
    


    <!-- http://purl.obolibrary.org/obo/GAZ_00020016 -->

    <owl:NamedIndividual rdf:about="http://purl.obolibrary.org/obo/GAZ_00020016">
        <rdf:type rdf:resource="http://purl.obolibrary.org/obo/ENVO_00000856"/>
        <obo:RO_0001025 rdf:resource="http://purl.obolibrary.org/obo/GAZ_00001207"/>
        <obo:IAO_0000115>A municipality.</obo:IAO_0000115>
        <oboInOwl:hasOBONamespace>GAZ</oboInOwl:hasOBONamespace>
        <oboInOwl:id>GAZ:00020016</oboInOwl:id>
        <rdfs:label>Grytubakkahreppur</rdfs:label>
    </owl:NamedIndividual>
    


    <!-- http://purl.obolibrary.org/obo/GAZ_00020017 -->

    <owl:NamedIndividual rdf:about="http://purl.obolibrary.org/obo/GAZ_00020017">
        <rdf:type rdf:resource="http://purl.obolibrary.org/obo/ENVO_00000856"/>
        <obo:RO_0001025 rdf:resource="http://purl.obolibrary.org/obo/GAZ_00001207"/>
        <obo:IAO_0000115>A municipality.</obo:IAO_0000115>
        <oboInOwl:hasOBONamespace>GAZ</oboInOwl:hasOBONamespace>
        <oboInOwl:id>GAZ:00020017</oboInOwl:id>
        <rdfs:label>Municipality of Horgarbyggd</rdfs:label>
    </owl:NamedIndividual>
    


    <!-- http://purl.obolibrary.org/obo/GAZ_00020018 -->

    <owl:NamedIndividual rdf:about="http://purl.obolibrary.org/obo/GAZ_00020018">
        <rdf:type rdf:resource="http://purl.obolibrary.org/obo/ENVO_00000856"/>
        <obo:RO_0001025 rdf:resource="http://purl.obolibrary.org/obo/GAZ_00001207"/>
        <obo:IAO_0000115>A municipality.</obo:IAO_0000115>
        <oboInOwl:hasOBONamespace>GAZ</oboInOwl:hasOBONamespace>
        <oboInOwl:id>GAZ:00020018</oboInOwl:id>
        <rdfs:label>Municipality of Langanesbyggd</rdfs:label>
    </owl:NamedIndividual>
    


    <!-- http://purl.obolibrary.org/obo/GAZ_00020019 -->

    <owl:NamedIndividual rdf:about="http://purl.obolibrary.org/obo/GAZ_00020019">
        <rdf:type rdf:resource="http://purl.obolibrary.org/obo/ENVO_00000856"/>
        <obo:RO_0001025 rdf:resource="http://purl.obolibrary.org/obo/GAZ_00001207"/>
        <obo:IAO_0000115>A municipality.</obo:IAO_0000115>
        <oboInOwl:hasOBONamespace>GAZ</oboInOwl:hasOBONamespace>
        <oboInOwl:id>GAZ:00020019</oboInOwl:id>
        <rdfs:label>Municipality of Nordurthing</rdfs:label>
    </owl:NamedIndividual>
    


    <!-- http://purl.obolibrary.org/obo/GAZ_00020020 -->

    <owl:NamedIndividual rdf:about="http://purl.obolibrary.org/obo/GAZ_00020020">
        <rdf:type rdf:resource="http://purl.obolibrary.org/obo/ENVO_00000856"/>
        <obo:RO_0001025 rdf:resource="http://purl.obolibrary.org/obo/GAZ_00001207"/>
        <obo:IAO_0000115>A municipality.</obo:IAO_0000115>
        <oboInOwl:hasOBONamespace>GAZ</oboInOwl:hasOBONamespace>
        <oboInOwl:id>GAZ:00020020</oboInOwl:id>
        <rdfs:label>Skutustadahreppur</rdfs:label>
    </owl:NamedIndividual>
    


    <!-- http://purl.obolibrary.org/obo/GAZ_00020021 -->

    <owl:NamedIndividual rdf:about="http://purl.obolibrary.org/obo/GAZ_00020021">
        <rdf:type rdf:resource="http://purl.obolibrary.org/obo/ENVO_00000856"/>
        <obo:RO_0001025 rdf:resource="http://purl.obolibrary.org/obo/GAZ_00001207"/>
        <obo:IAO_0000115>A municipality.</obo:IAO_0000115>
        <oboInOwl:hasOBONamespace>GAZ</oboInOwl:hasOBONamespace>
        <oboInOwl:id>GAZ:00020021</oboInOwl:id>
        <rdfs:label>Svalbardshreppur</rdfs:label>
    </owl:NamedIndividual>
    


    <!-- http://purl.obolibrary.org/obo/GAZ_00020022 -->

    <owl:NamedIndividual rdf:about="http://purl.obolibrary.org/obo/GAZ_00020022">
        <rdf:type rdf:resource="http://purl.obolibrary.org/obo/ENVO_00000856"/>
        <obo:RO_0001025 rdf:resource="http://purl.obolibrary.org/obo/GAZ_00001207"/>
        <obo:IAO_0000115>A municipality.</obo:IAO_0000115>
        <oboInOwl:hasOBONamespace>GAZ</oboInOwl:hasOBONamespace>
        <oboInOwl:id>GAZ:00020022</oboInOwl:id>
        <rdfs:label>Svalbardsstrandarhreppur</rdfs:label>
    </owl:NamedIndividual>
    


    <!-- http://purl.obolibrary.org/obo/GAZ_00020023 -->

    <owl:NamedIndividual rdf:about="http://purl.obolibrary.org/obo/GAZ_00020023">
        <rdf:type rdf:resource="http://purl.obolibrary.org/obo/ENVO_00000856"/>
        <obo:RO_0001025 rdf:resource="http://purl.obolibrary.org/obo/GAZ_00001207"/>
        <obo:IAO_0000115>A municipality.</obo:IAO_0000115>
        <oboInOwl:hasOBONamespace>GAZ</oboInOwl:hasOBONamespace>
        <oboInOwl:id>GAZ:00020023</oboInOwl:id>
        <rdfs:label>Municipality of Thingeyjarsveit</rdfs:label>
    </owl:NamedIndividual>
    


    <!-- http://purl.obolibrary.org/obo/GAZ_00020024 -->

    <owl:NamedIndividual rdf:about="http://purl.obolibrary.org/obo/GAZ_00020024">
        <rdf:type rdf:resource="http://purl.obolibrary.org/obo/ENVO_00000856"/>
        <obo:RO_0001025 rdf:resource="http://purl.obolibrary.org/obo/GAZ_00001207"/>
        <obo:IAO_0000115>A municipality.</obo:IAO_0000115>
        <oboInOwl:hasOBONamespace>GAZ</oboInOwl:hasOBONamespace>
        <oboInOwl:id>GAZ:00020024</oboInOwl:id>
        <rdfs:label>Tjorneshreppur</rdfs:label>
    </owl:NamedIndividual>
    


    <!-- http://purl.obolibrary.org/obo/GAZ_00020025 -->

    <owl:NamedIndividual rdf:about="http://purl.obolibrary.org/obo/GAZ_00020025">
        <rdf:type rdf:resource="http://purl.obolibrary.org/obo/ENVO_00000856"/>
        <obo:RO_0001025 rdf:resource="http://purl.obolibrary.org/obo/GAZ_00001202"/>
        <obo:IAO_0000115>A municipality.</obo:IAO_0000115>
        <oboInOwl:hasOBONamespace>GAZ</oboInOwl:hasOBONamespace>
        <oboInOwl:id>GAZ:00020025</oboInOwl:id>
        <rdfs:label>Akrahreppur</rdfs:label>
    </owl:NamedIndividual>
    


    <!-- http://purl.obolibrary.org/obo/GAZ_00020026 -->

    <owl:NamedIndividual rdf:about="http://purl.obolibrary.org/obo/GAZ_00020026">
        <rdf:type rdf:resource="http://purl.obolibrary.org/obo/ENVO_00000856"/>
        <obo:RO_0001025 rdf:resource="http://purl.obolibrary.org/obo/GAZ_00001202"/>
        <obo:IAO_0000115>A municipality.</obo:IAO_0000115>
        <oboInOwl:hasOBONamespace>GAZ</oboInOwl:hasOBONamespace>
        <oboInOwl:id>GAZ:00020026</oboInOwl:id>
        <rdfs:label>Municipality of Blonduossbaer</rdfs:label>
    </owl:NamedIndividual>
    


    <!-- http://purl.obolibrary.org/obo/GAZ_00020028 -->

    <owl:NamedIndividual rdf:about="http://purl.obolibrary.org/obo/GAZ_00020028">
        <rdf:type rdf:resource="http://purl.obolibrary.org/obo/ENVO_00000856"/>
        <obo:RO_0001025 rdf:resource="http://purl.obolibrary.org/obo/GAZ_00001202"/>
        <obo:IAO_0000115>A municipality.</obo:IAO_0000115>
        <oboInOwl:hasOBONamespace>GAZ</oboInOwl:hasOBONamespace>
        <oboInOwl:id>GAZ:00020028</oboInOwl:id>
        <rdfs:label>Municipality of Hunathing vestra</rdfs:label>
    </owl:NamedIndividual>
    


    <!-- http://purl.obolibrary.org/obo/GAZ_00020029 -->

    <owl:NamedIndividual rdf:about="http://purl.obolibrary.org/obo/GAZ_00020029">
        <rdf:type rdf:resource="http://purl.obolibrary.org/obo/ENVO_00000856"/>
        <obo:RO_0001025 rdf:resource="http://purl.obolibrary.org/obo/GAZ_00001202"/>
        <obo:IAO_0000115>A municipality.</obo:IAO_0000115>
        <oboInOwl:hasOBONamespace>GAZ</oboInOwl:hasOBONamespace>
        <oboInOwl:id>GAZ:00020029</oboInOwl:id>
        <rdfs:label>Hunavatnshreppur</rdfs:label>
    </owl:NamedIndividual>
    


    <!-- http://purl.obolibrary.org/obo/GAZ_00020030 -->

    <owl:NamedIndividual rdf:about="http://purl.obolibrary.org/obo/GAZ_00020030">
        <rdf:type rdf:resource="http://purl.obolibrary.org/obo/ENVO_00000856"/>
        <obo:RO_0001025 rdf:resource="http://purl.obolibrary.org/obo/GAZ_00001202"/>
        <obo:IAO_0000115>A municipality.</obo:IAO_0000115>
        <oboInOwl:hasOBONamespace>GAZ</oboInOwl:hasOBONamespace>
        <oboInOwl:id>GAZ:00020030</oboInOwl:id>
        <rdfs:label>Municipality of Skagabyggd</rdfs:label>
    </owl:NamedIndividual>
    


    <!-- http://purl.obolibrary.org/obo/GAZ_00020031 -->

    <owl:NamedIndividual rdf:about="http://purl.obolibrary.org/obo/GAZ_00020031">
        <rdf:type rdf:resource="http://purl.obolibrary.org/obo/ENVO_00000856"/>
        <obo:RO_0001025 rdf:resource="http://purl.obolibrary.org/obo/GAZ_00001202"/>
        <obo:IAO_0000115>A municipality.</obo:IAO_0000115>
        <oboInOwl:hasOBONamespace>GAZ</oboInOwl:hasOBONamespace>
        <oboInOwl:id>GAZ:00020031</oboInOwl:id>
        <rdfs:label>Sveitarfelagid Skagafjoerdur</rdfs:label>
    </owl:NamedIndividual>
    


    <!-- http://purl.obolibrary.org/obo/GAZ_00020032 -->

    <owl:NamedIndividual rdf:about="http://purl.obolibrary.org/obo/GAZ_00020032">
        <rdf:type rdf:resource="http://purl.obolibrary.org/obo/ENVO_00000856"/>
        <obo:RO_0001025 rdf:resource="http://purl.obolibrary.org/obo/GAZ_00008175"/>
        <obo:IAO_0000115>A municipality on the peninsula of Reykjanes at the south-western coast of Iceland.</obo:IAO_0000115>
        <oboInOwl:hasOBONamespace>GAZ</oboInOwl:hasOBONamespace>
        <oboInOwl:id>GAZ:00020032</oboInOwl:id>
        <rdfs:label>Municipality of Grindavikurbaer</rdfs:label>
    </owl:NamedIndividual>
    


    <!-- http://purl.obolibrary.org/obo/GAZ_00020033 -->

    <owl:NamedIndividual rdf:about="http://purl.obolibrary.org/obo/GAZ_00020033">
        <rdf:type rdf:resource="http://purl.obolibrary.org/obo/ENVO_00000856"/>
        <obo:RO_0001025 rdf:resource="http://purl.obolibrary.org/obo/GAZ_00008175"/>
        <obo:IAO_0000115>A municipality.</obo:IAO_0000115>
        <oboInOwl:hasOBONamespace>GAZ</oboInOwl:hasOBONamespace>
        <oboInOwl:id>GAZ:00020033</oboInOwl:id>
        <rdfs:label>Municipality of Reykjanesbaer</rdfs:label>
    </owl:NamedIndividual>
    


    <!-- http://purl.obolibrary.org/obo/GAZ_00020034 -->

    <owl:NamedIndividual rdf:about="http://purl.obolibrary.org/obo/GAZ_00020034">
        <rdf:type rdf:resource="http://purl.obolibrary.org/obo/ENVO_00000856"/>
        <obo:RO_0001025 rdf:resource="http://purl.obolibrary.org/obo/GAZ_00008175"/>
        <obo:IAO_0000115>A municipality.</obo:IAO_0000115>
        <oboInOwl:hasOBONamespace>GAZ</oboInOwl:hasOBONamespace>
        <oboInOwl:id>GAZ:00020034</oboInOwl:id>
        <rdfs:label>Municipality of Sandgerdisbaer</rdfs:label>
    </owl:NamedIndividual>
    


    <!-- http://purl.obolibrary.org/obo/GAZ_00020035 -->

    <owl:NamedIndividual rdf:about="http://purl.obolibrary.org/obo/GAZ_00020035">
        <rdf:type rdf:resource="http://purl.obolibrary.org/obo/ENVO_00000856"/>
        <obo:RO_0001025 rdf:resource="http://purl.obolibrary.org/obo/GAZ_00008175"/>
        <obo:IAO_0000115>A municipality.</obo:IAO_0000115>
        <oboInOwl:hasOBONamespace>GAZ</oboInOwl:hasOBONamespace>
        <oboInOwl:id>GAZ:00020035</oboInOwl:id>
        <rdfs:label>Sveitarfelagid Gardur</rdfs:label>
    </owl:NamedIndividual>
    


    <!-- http://purl.obolibrary.org/obo/GAZ_00020036 -->

    <owl:NamedIndividual rdf:about="http://purl.obolibrary.org/obo/GAZ_00020036">
        <rdf:type rdf:resource="http://purl.obolibrary.org/obo/ENVO_00000856"/>
        <obo:RO_0001025 rdf:resource="http://purl.obolibrary.org/obo/GAZ_00008175"/>
        <obo:IAO_0000115>A municipality.</obo:IAO_0000115>
        <oboInOwl:hasOBONamespace>GAZ</oboInOwl:hasOBONamespace>
        <oboInOwl:id>GAZ:00020036</oboInOwl:id>
        <rdfs:label>Sveitarfelagid Vogar</rdfs:label>
    </owl:NamedIndividual>
    


    <!-- http://purl.obolibrary.org/obo/GAZ_00020037 -->

    <owl:NamedIndividual rdf:about="http://purl.obolibrary.org/obo/GAZ_00020037">
        <rdf:type rdf:resource="http://purl.obolibrary.org/obo/ENVO_00000856"/>
        <obo:RO_0001025 rdf:resource="http://purl.obolibrary.org/obo/GAZ_00001204"/>
        <obo:IAO_0000115>A municipality.</obo:IAO_0000115>
        <oboInOwl:hasOBONamespace>GAZ</oboInOwl:hasOBONamespace>
        <oboInOwl:id>GAZ:00020037</oboInOwl:id>
        <rdfs:label>Municipality of Asahreppur</rdfs:label>
    </owl:NamedIndividual>
    


    <!-- http://purl.obolibrary.org/obo/GAZ_00020038 -->

    <owl:NamedIndividual rdf:about="http://purl.obolibrary.org/obo/GAZ_00020038">
        <rdf:type rdf:resource="http://purl.obolibrary.org/obo/ENVO_00000856"/>
        <obo:RO_0001025 rdf:resource="http://purl.obolibrary.org/obo/GAZ_00001204"/>
        <obo:IAO_0000115>A municipality.</obo:IAO_0000115>
        <oboInOwl:hasOBONamespace>GAZ</oboInOwl:hasOBONamespace>
        <oboInOwl:id>GAZ:00020038</oboInOwl:id>
        <rdfs:label>Municipality of Blaskogabyggd</rdfs:label>
    </owl:NamedIndividual>
    


    <!-- http://purl.obolibrary.org/obo/GAZ_00020039 -->

    <owl:NamedIndividual rdf:about="http://purl.obolibrary.org/obo/GAZ_00020039">
        <rdf:type rdf:resource="http://purl.obolibrary.org/obo/ENVO_00000856"/>
        <obo:RO_0001025 rdf:resource="http://purl.obolibrary.org/obo/GAZ_00001204"/>
        <obo:IAO_0000115>A municipality.</obo:IAO_0000115>
        <oboInOwl:hasOBONamespace>GAZ</oboInOwl:hasOBONamespace>
        <oboInOwl:id>GAZ:00020039</oboInOwl:id>
        <rdfs:label>Floahreppur</rdfs:label>
    </owl:NamedIndividual>
    


    <!-- http://purl.obolibrary.org/obo/GAZ_00020040 -->

    <owl:NamedIndividual rdf:about="http://purl.obolibrary.org/obo/GAZ_00020040">
        <rdf:type rdf:resource="http://purl.obolibrary.org/obo/ENVO_00000856"/>
        <obo:RO_0001025 rdf:resource="http://purl.obolibrary.org/obo/GAZ_00001204"/>
        <obo:IAO_0000115>A municipality.</obo:IAO_0000115>
        <oboInOwl:hasOBONamespace>GAZ</oboInOwl:hasOBONamespace>
        <oboInOwl:id>GAZ:00020040</oboInOwl:id>
        <rdfs:label>Grimsnes-og Grafningshreppur</rdfs:label>
    </owl:NamedIndividual>
    


    <!-- http://purl.obolibrary.org/obo/GAZ_00020041 -->

    <owl:NamedIndividual rdf:about="http://purl.obolibrary.org/obo/GAZ_00020041">
        <rdf:type rdf:resource="http://purl.obolibrary.org/obo/ENVO_00000856"/>
        <obo:RO_0001025 rdf:resource="http://purl.obolibrary.org/obo/GAZ_00001204"/>
        <obo:IAO_0000115>A municipality.</obo:IAO_0000115>
        <oboInOwl:hasOBONamespace>GAZ</oboInOwl:hasOBONamespace>
        <oboInOwl:id>GAZ:00020041</oboInOwl:id>
        <rdfs:label>Hrunamannahreppur</rdfs:label>
    </owl:NamedIndividual>
    


    <!-- http://purl.obolibrary.org/obo/GAZ_00020042 -->

    <owl:NamedIndividual rdf:about="http://purl.obolibrary.org/obo/GAZ_00020042">
        <rdf:type rdf:resource="http://purl.obolibrary.org/obo/ENVO_00000856"/>
        <obo:RO_0001025 rdf:resource="http://purl.obolibrary.org/obo/GAZ_00001204"/>
        <obo:IAO_0000115>A municipality.</obo:IAO_0000115>
        <oboInOwl:hasOBONamespace>GAZ</oboInOwl:hasOBONamespace>
        <oboInOwl:id>GAZ:00020042</oboInOwl:id>
        <rdfs:label>Municipality of Hveragerdisbaer</rdfs:label>
    </owl:NamedIndividual>
    


    <!-- http://purl.obolibrary.org/obo/GAZ_00020043 -->

    <owl:NamedIndividual rdf:about="http://purl.obolibrary.org/obo/GAZ_00020043">
        <rdf:type rdf:resource="http://purl.obolibrary.org/obo/ENVO_00000856"/>
        <obo:RO_0001025 rdf:resource="http://purl.obolibrary.org/obo/GAZ_00001204"/>
        <obo:IAO_0000115>A municipality.</obo:IAO_0000115>
        <oboInOwl:hasOBONamespace>GAZ</oboInOwl:hasOBONamespace>
        <oboInOwl:id>GAZ:00020043</oboInOwl:id>
        <rdfs:label>Myrdalshreppur</rdfs:label>
    </owl:NamedIndividual>
    


    <!-- http://purl.obolibrary.org/obo/GAZ_00020044 -->

    <owl:NamedIndividual rdf:about="http://purl.obolibrary.org/obo/GAZ_00020044">
        <rdf:type rdf:resource="http://purl.obolibrary.org/obo/ENVO_00000856"/>
        <obo:RO_0001025 rdf:resource="http://purl.obolibrary.org/obo/GAZ_00001204"/>
        <obo:IAO_0000115>A municipality.</obo:IAO_0000115>
        <oboInOwl:hasOBONamespace>GAZ</oboInOwl:hasOBONamespace>
        <oboInOwl:id>GAZ:00020044</oboInOwl:id>
        <rdfs:label>Municipality of Rangarthing eystra</rdfs:label>
    </owl:NamedIndividual>
    


    <!-- http://purl.obolibrary.org/obo/GAZ_00020045 -->

    <owl:NamedIndividual rdf:about="http://purl.obolibrary.org/obo/GAZ_00020045">
        <rdf:type rdf:resource="http://purl.obolibrary.org/obo/ENVO_00000856"/>
        <obo:RO_0001025 rdf:resource="http://purl.obolibrary.org/obo/GAZ_00001204"/>
        <obo:IAO_0000115>A municipality.</obo:IAO_0000115>
        <oboInOwl:hasOBONamespace>GAZ</oboInOwl:hasOBONamespace>
        <oboInOwl:id>GAZ:00020045</oboInOwl:id>
        <rdfs:label>Municipality of Rangarthing ytra</rdfs:label>
    </owl:NamedIndividual>
    


    <!-- http://purl.obolibrary.org/obo/GAZ_00020046 -->

    <owl:NamedIndividual rdf:about="http://purl.obolibrary.org/obo/GAZ_00020046">
        <rdf:type rdf:resource="http://purl.obolibrary.org/obo/ENVO_00000856"/>
        <obo:RO_0001025 rdf:resource="http://purl.obolibrary.org/obo/GAZ_00001204"/>
        <obo:IAO_0000115>A municipality.</obo:IAO_0000115>
        <oboInOwl:hasOBONamespace>GAZ</oboInOwl:hasOBONamespace>
        <oboInOwl:id>GAZ:00020046</oboInOwl:id>
        <rdfs:label>Skaftarhreppur</rdfs:label>
    </owl:NamedIndividual>
    


    <!-- http://purl.obolibrary.org/obo/GAZ_00020047 -->

    <owl:NamedIndividual rdf:about="http://purl.obolibrary.org/obo/GAZ_00020047">
        <rdf:type rdf:resource="http://purl.obolibrary.org/obo/ENVO_00000856"/>
        <obo:RO_0001025 rdf:resource="http://purl.obolibrary.org/obo/GAZ_00001204"/>
        <obo:IAO_0000115>A municipality.</obo:IAO_0000115>
        <oboInOwl:hasOBONamespace>GAZ</oboInOwl:hasOBONamespace>
        <oboInOwl:id>GAZ:00020047</oboInOwl:id>
        <rdfs:label>Skeida-og Gnupverjahreppur</rdfs:label>
    </owl:NamedIndividual>
    


    <!-- http://purl.obolibrary.org/obo/GAZ_00020048 -->

    <owl:NamedIndividual rdf:about="http://purl.obolibrary.org/obo/GAZ_00020048">
        <rdf:type rdf:resource="http://purl.obolibrary.org/obo/ENVO_00000856"/>
        <obo:RO_0001025 rdf:resource="http://purl.obolibrary.org/obo/GAZ_00001204"/>
        <obo:IAO_0000115>A municipality.</obo:IAO_0000115>
        <oboInOwl:hasOBONamespace>GAZ</oboInOwl:hasOBONamespace>
        <oboInOwl:id>GAZ:00020048</oboInOwl:id>
        <rdfs:label>Sveitarfelagid Olfus</rdfs:label>
    </owl:NamedIndividual>
    


    <!-- http://purl.obolibrary.org/obo/GAZ_00020049 -->

    <owl:NamedIndividual rdf:about="http://purl.obolibrary.org/obo/GAZ_00020049">
        <rdf:type rdf:resource="http://purl.obolibrary.org/obo/ENVO_00000856"/>
        <obo:RO_0001025 rdf:resource="http://purl.obolibrary.org/obo/GAZ_00145764"/>
        <obo:IAO_0000115>A municipality.</obo:IAO_0000115>
        <oboInOwl:hasOBONamespace>GAZ</oboInOwl:hasOBONamespace>
        <oboInOwl:id>GAZ:00020049</oboInOwl:id>
        <rdfs:label>Arneshreppur</rdfs:label>
    </owl:NamedIndividual>
    


    <!-- http://purl.obolibrary.org/obo/GAZ_00020050 -->

    <owl:NamedIndividual rdf:about="http://purl.obolibrary.org/obo/GAZ_00020050">
        <rdf:type rdf:resource="http://purl.obolibrary.org/obo/ENVO_00000856"/>
        <obo:RO_0001025 rdf:resource="http://purl.obolibrary.org/obo/GAZ_00145764"/>
        <obo:IAO_0000115>A municipality.</obo:IAO_0000115>
        <oboInOwl:hasOBONamespace>GAZ</oboInOwl:hasOBONamespace>
        <oboInOwl:id>GAZ:00020050</oboInOwl:id>
        <rdfs:label>Baejarhreppur</rdfs:label>
    </owl:NamedIndividual>
    


    <!-- http://purl.obolibrary.org/obo/GAZ_00020051 -->

    <owl:NamedIndividual rdf:about="http://purl.obolibrary.org/obo/GAZ_00020051">
        <rdf:type rdf:resource="http://purl.obolibrary.org/obo/ENVO_00000856"/>
        <obo:RO_0001025 rdf:resource="http://purl.obolibrary.org/obo/GAZ_00145764"/>
        <obo:IAO_0000115>A municipality.</obo:IAO_0000115>
        <oboInOwl:hasOBONamespace>GAZ</oboInOwl:hasOBONamespace>
        <oboInOwl:id>GAZ:00020051</oboInOwl:id>
        <rdfs:label>Municipality of Bolungarvikurkaupstadur</rdfs:label>
    </owl:NamedIndividual>
    


    <!-- http://purl.obolibrary.org/obo/GAZ_00020052 -->

    <owl:NamedIndividual rdf:about="http://purl.obolibrary.org/obo/GAZ_00020052">
        <rdf:type rdf:resource="http://purl.obolibrary.org/obo/ENVO_00000856"/>
        <obo:RO_0001025 rdf:resource="http://purl.obolibrary.org/obo/GAZ_00145764"/>
        <obo:IAO_0000115>A municipality.</obo:IAO_0000115>
        <oboInOwl:hasOBONamespace>GAZ</oboInOwl:hasOBONamespace>
        <oboInOwl:id>GAZ:00020052</oboInOwl:id>
        <rdfs:label>Municipality of Isafjardarbaer</rdfs:label>
    </owl:NamedIndividual>
    


    <!-- http://purl.obolibrary.org/obo/GAZ_00020053 -->

    <owl:NamedIndividual rdf:about="http://purl.obolibrary.org/obo/GAZ_00020053">
        <rdf:type rdf:resource="http://purl.obolibrary.org/obo/ENVO_00000856"/>
        <obo:RO_0001025 rdf:resource="http://purl.obolibrary.org/obo/GAZ_00145764"/>
        <obo:IAO_0000115>A municipality.</obo:IAO_0000115>
        <oboInOwl:hasOBONamespace>GAZ</oboInOwl:hasOBONamespace>
        <oboInOwl:id>GAZ:00020053</oboInOwl:id>
        <rdfs:label>Kaldrananeshreppur</rdfs:label>
    </owl:NamedIndividual>
    


    <!-- http://purl.obolibrary.org/obo/GAZ_00020054 -->

    <owl:NamedIndividual rdf:about="http://purl.obolibrary.org/obo/GAZ_00020054">
        <rdf:type rdf:resource="http://purl.obolibrary.org/obo/ENVO_00000856"/>
        <obo:RO_0001025 rdf:resource="http://purl.obolibrary.org/obo/GAZ_00145764"/>
        <obo:IAO_0000115>A municipality.</obo:IAO_0000115>
        <oboInOwl:hasOBONamespace>GAZ</oboInOwl:hasOBONamespace>
        <oboInOwl:id>GAZ:00020054</oboInOwl:id>
        <rdfs:label>Reykholahreppur</rdfs:label>
    </owl:NamedIndividual>
    


    <!-- http://purl.obolibrary.org/obo/GAZ_00020055 -->

    <owl:NamedIndividual rdf:about="http://purl.obolibrary.org/obo/GAZ_00020055">
        <rdf:type rdf:resource="http://purl.obolibrary.org/obo/ENVO_00000856"/>
        <obo:RO_0001025 rdf:resource="http://purl.obolibrary.org/obo/GAZ_00145764"/>
        <obo:IAO_0000115>A municipality.</obo:IAO_0000115>
        <oboInOwl:hasOBONamespace>GAZ</oboInOwl:hasOBONamespace>
        <oboInOwl:id>GAZ:00020055</oboInOwl:id>
        <rdfs:label>Municipality of Strandabyggd</rdfs:label>
    </owl:NamedIndividual>
    


    <!-- http://purl.obolibrary.org/obo/GAZ_00020056 -->

    <owl:NamedIndividual rdf:about="http://purl.obolibrary.org/obo/GAZ_00020056">
        <rdf:type rdf:resource="http://purl.obolibrary.org/obo/ENVO_00000856"/>
        <obo:RO_0001025 rdf:resource="http://purl.obolibrary.org/obo/GAZ_00145764"/>
        <obo:IAO_0000115>A municipality.</obo:IAO_0000115>
        <oboInOwl:hasOBONamespace>GAZ</oboInOwl:hasOBONamespace>
        <oboInOwl:id>GAZ:00020056</oboInOwl:id>
        <rdfs:label>Sudavikurhreppur</rdfs:label>
    </owl:NamedIndividual>
    


    <!-- http://purl.obolibrary.org/obo/GAZ_00020057 -->

    <owl:NamedIndividual rdf:about="http://purl.obolibrary.org/obo/GAZ_00020057">
        <rdf:type rdf:resource="http://purl.obolibrary.org/obo/ENVO_00000856"/>
        <obo:RO_0001025 rdf:resource="http://purl.obolibrary.org/obo/GAZ_00145764"/>
        <obo:IAO_0000115>A municipality.</obo:IAO_0000115>
        <oboInOwl:hasOBONamespace>GAZ</oboInOwl:hasOBONamespace>
        <oboInOwl:id>GAZ:00020057</oboInOwl:id>
        <rdfs:label>Talknafjardarhreppur</rdfs:label>
    </owl:NamedIndividual>
    


    <!-- http://purl.obolibrary.org/obo/GAZ_00020058 -->

    <owl:NamedIndividual rdf:about="http://purl.obolibrary.org/obo/GAZ_00020058">
        <rdf:type rdf:resource="http://purl.obolibrary.org/obo/ENVO_00000856"/>
        <obo:RO_0001025 rdf:resource="http://purl.obolibrary.org/obo/GAZ_00145764"/>
        <obo:IAO_0000115>A municipality.</obo:IAO_0000115>
        <oboInOwl:hasOBONamespace>GAZ</oboInOwl:hasOBONamespace>
        <oboInOwl:id>GAZ:00020058</oboInOwl:id>
        <rdfs:label>Municipality of Vesturbyggd</rdfs:label>
    </owl:NamedIndividual>
    


    <!-- http://purl.obolibrary.org/obo/GAZ_00020059 -->

    <owl:NamedIndividual rdf:about="http://purl.obolibrary.org/obo/GAZ_00020059">
        <rdf:type rdf:resource="http://purl.obolibrary.org/obo/ENVO_00000856"/>
        <obo:RO_0001025 rdf:resource="http://purl.obolibrary.org/obo/GAZ_00001206"/>
        <obo:IAO_0000115>A municipality.</obo:IAO_0000115>
        <oboInOwl:hasOBONamespace>GAZ</oboInOwl:hasOBONamespace>
        <oboInOwl:id>GAZ:00020059</oboInOwl:id>
        <rdfs:label>Municipality of Akraneskaupstadur</rdfs:label>
    </owl:NamedIndividual>
    


    <!-- http://purl.obolibrary.org/obo/GAZ_00020060 -->

    <owl:NamedIndividual rdf:about="http://purl.obolibrary.org/obo/GAZ_00020060">
        <rdf:type rdf:resource="http://purl.obolibrary.org/obo/ENVO_00000856"/>
        <obo:RO_0001025 rdf:resource="http://purl.obolibrary.org/obo/GAZ_00001206"/>
        <obo:IAO_0000115>A municipality.</obo:IAO_0000115>
        <oboInOwl:hasOBONamespace>GAZ</oboInOwl:hasOBONamespace>
        <oboInOwl:id>GAZ:00020060</oboInOwl:id>
        <rdfs:label>Municipality of Borgarbyggd</rdfs:label>
    </owl:NamedIndividual>
    


    <!-- http://purl.obolibrary.org/obo/GAZ_00020061 -->

    <owl:NamedIndividual rdf:about="http://purl.obolibrary.org/obo/GAZ_00020061">
        <rdf:type rdf:resource="http://purl.obolibrary.org/obo/ENVO_00000856"/>
        <obo:RO_0001025 rdf:resource="http://purl.obolibrary.org/obo/GAZ_00001206"/>
        <obo:IAO_0000115>A municipality.</obo:IAO_0000115>
        <oboInOwl:hasOBONamespace>GAZ</oboInOwl:hasOBONamespace>
        <oboInOwl:id>GAZ:00020061</oboInOwl:id>
        <rdfs:label>Municipality of Dalabyggd</rdfs:label>
    </owl:NamedIndividual>
    


    <!-- http://purl.obolibrary.org/obo/GAZ_00020062 -->

    <owl:NamedIndividual rdf:about="http://purl.obolibrary.org/obo/GAZ_00020062">
        <rdf:type rdf:resource="http://purl.obolibrary.org/obo/ENVO_00000856"/>
        <obo:RO_0001025 rdf:resource="http://purl.obolibrary.org/obo/GAZ_00062086"/>
        <obo:IAO_0000115>A municipality.</obo:IAO_0000115>
        <oboInOwl:hasOBONamespace>GAZ</oboInOwl:hasOBONamespace>
        <oboInOwl:id>GAZ:00020062</oboInOwl:id>
        <rdfs:label>Eyja-og Miklaholtshreppur</rdfs:label>
    </owl:NamedIndividual>
    


    <!-- http://purl.obolibrary.org/obo/GAZ_00020063 -->

    <owl:NamedIndividual rdf:about="http://purl.obolibrary.org/obo/GAZ_00020063">
        <rdf:type rdf:resource="http://purl.obolibrary.org/obo/ENVO_00000856"/>
        <obo:RO_0001025 rdf:resource="http://purl.obolibrary.org/obo/GAZ_00062086"/>
        <obo:IAO_0000115>A municipality.</obo:IAO_0000115>
        <oboInOwl:hasOBONamespace>GAZ</oboInOwl:hasOBONamespace>
        <oboInOwl:id>GAZ:00020063</oboInOwl:id>
        <rdfs:label>Municipality of Grundarfjardarbaer</rdfs:label>
    </owl:NamedIndividual>
    


    <!-- http://purl.obolibrary.org/obo/GAZ_00020064 -->

    <owl:NamedIndividual rdf:about="http://purl.obolibrary.org/obo/GAZ_00020064">
        <rdf:type rdf:resource="http://purl.obolibrary.org/obo/ENVO_00000856"/>
        <obo:RO_0001025 rdf:resource="http://purl.obolibrary.org/obo/GAZ_00062086"/>
        <obo:IAO_0000115>A municipality.</obo:IAO_0000115>
        <oboInOwl:hasOBONamespace>GAZ</oboInOwl:hasOBONamespace>
        <oboInOwl:id>GAZ:00020064</oboInOwl:id>
        <rdfs:label>Municipality of Helgafellssveit</rdfs:label>
    </owl:NamedIndividual>
    


    <!-- http://purl.obolibrary.org/obo/GAZ_00020065 -->

    <owl:NamedIndividual rdf:about="http://purl.obolibrary.org/obo/GAZ_00020065">
        <rdf:type rdf:resource="http://purl.obolibrary.org/obo/ENVO_00000856"/>
        <obo:RO_0001025 rdf:resource="http://purl.obolibrary.org/obo/GAZ_00001206"/>
        <obo:IAO_0000115>A municipality.</obo:IAO_0000115>
        <oboInOwl:hasOBONamespace>GAZ</oboInOwl:hasOBONamespace>
        <oboInOwl:id>GAZ:00020065</oboInOwl:id>
        <rdfs:label>Municipality of Hvalfjardarsveit</rdfs:label>
    </owl:NamedIndividual>
    


    <!-- http://purl.obolibrary.org/obo/GAZ_00020066 -->

    <owl:NamedIndividual rdf:about="http://purl.obolibrary.org/obo/GAZ_00020066">
        <rdf:type rdf:resource="http://purl.obolibrary.org/obo/ENVO_00000856"/>
        <obo:RO_0001025 rdf:resource="http://purl.obolibrary.org/obo/GAZ_00001206"/>
        <obo:IAO_0000115>A municipality.</obo:IAO_0000115>
        <oboInOwl:hasOBONamespace>GAZ</oboInOwl:hasOBONamespace>
        <oboInOwl:id>GAZ:00020066</oboInOwl:id>
        <rdfs:label>Municipality of Skorradalshreppur</rdfs:label>
    </owl:NamedIndividual>
    


    <!-- http://purl.obolibrary.org/obo/GAZ_00020067 -->

    <owl:NamedIndividual rdf:about="http://purl.obolibrary.org/obo/GAZ_00020067">
        <rdf:type rdf:resource="http://purl.obolibrary.org/obo/ENVO_00000856"/>
        <obo:RO_0001025 rdf:resource="http://purl.obolibrary.org/obo/GAZ_00062086"/>
        <obo:IAO_0000115>A municipality.</obo:IAO_0000115>
        <oboInOwl:hasOBONamespace>GAZ</oboInOwl:hasOBONamespace>
        <oboInOwl:id>GAZ:00020067</oboInOwl:id>
        <rdfs:label>Municipality of Snaefellsbaer</rdfs:label>
    </owl:NamedIndividual>
    


    <!-- http://purl.obolibrary.org/obo/GAZ_00020068 -->

    <owl:NamedIndividual rdf:about="http://purl.obolibrary.org/obo/GAZ_00020068">
        <rdf:type rdf:resource="http://purl.obolibrary.org/obo/ENVO_00000856"/>
        <obo:RO_0001025 rdf:resource="http://purl.obolibrary.org/obo/GAZ_00062086"/>
        <obo:IAO_0000115>A municipality.</obo:IAO_0000115>
        <oboInOwl:hasOBONamespace>GAZ</oboInOwl:hasOBONamespace>
        <oboInOwl:id>GAZ:00020068</oboInOwl:id>
        <rdfs:label>Municipality of Stykkisholmsbaer</rdfs:label>
    </owl:NamedIndividual>
    


    <!-- http://purl.obolibrary.org/obo/GAZ_00051977 -->

    <owl:NamedIndividual rdf:about="http://purl.obolibrary.org/obo/GAZ_00051977">
        <obo:RO_0001025 rdf:resource="http://purl.obolibrary.org/obo/GAZ_00001204"/>
        <obo:RO_0001025 rdf:resource="http://purl.obolibrary.org/obo/GAZ_00280523"/>
        <obo:IAO_0000115>A mostly submarine volcanic system is the southernmost and youngest volcanic center of the eastern volcanic zone that cuts across east-central Iceland. It consists of a roughly 30 x 40 km group of basaltic volcanic islands and submarine cones occupying a shallow shelf off the south coast of Iceland. Vestmannaeyjar was the site of two of Iceland&apos;s most noted 20th-century eruptions. The new island of Surtsey grew from the ocean floor during 1963-67. The island of Heimaey, 20 km to the NE, was the site of dramatic eruptions in 1973 during which lava flows partially overran the town of Vestmannaeyjar and threatened its harbor. Several other volcanoes have erupted during historical time. Twenty-two postglacial eruption sites are known in the Vestmannaeyjar system, and all ten subaerial vents on Heimaey are of Holocene age.</obo:IAO_0000115>
        <oboInOwl:hasOBONamespace>GAZ</oboInOwl:hasOBONamespace>
        <oboInOwl:id>GAZ:00051977</oboInOwl:id>
        <rdfs:label>Vestmannaeyjar Volcanic System</rdfs:label>
    </owl:NamedIndividual>
    


    <!-- http://purl.obolibrary.org/obo/GAZ_00051978 -->

    <owl:NamedIndividual rdf:about="http://purl.obolibrary.org/obo/GAZ_00051978">
        <obo:RO_0001025 rdf:resource="http://purl.obolibrary.org/obo/GAZ_00089839"/>
        <obo:IAO_0000115>A stratovolcano that anchors the western tip of the isolated Snaefellsnes Peninsula in western Iceland. Numerous pyroclastic cones dot the flanks of the 1448 m high stratovolcano, the only large central volcano in this part of Iceland. Lower-flank craters produced basaltic lava flows and upper-flank craters intermediate-to-silicic material. Holocene lava flows extend to the sea over the entire western half of the volcano. Several Holocene silicic eruptions have originated from the summit crater. The latest dated eruption took place about 1750 years ago; several lava flows may be even younger.</obo:IAO_0000115>
        <oboInOwl:hasOBONamespace>GAZ</oboInOwl:hasOBONamespace>
        <oboInOwl:id>GAZ:00051978</oboInOwl:id>
        <rdfs:label>Snaefellsokull [volcano]</rdfs:label>
    </owl:NamedIndividual>
    


    <!-- http://purl.obolibrary.org/obo/GAZ_00051979 -->

    <owl:NamedIndividual rdf:about="http://purl.obolibrary.org/obo/GAZ_00051979">
        <rdf:type rdf:resource="http://purl.obolibrary.org/obo/ENVO_00000354"/>
        <obo:RO_0001025 rdf:resource="http://purl.obolibrary.org/obo/GAZ_00062086"/>
        <obo:IAO_0000115>A volcanic system that consists of a chain of small alkali olivine basaltic cinder cones and vents along a WNW-ESE line cutting across the central Snaefellsnes Peninsula in western Iceland. The slightly arcuate line of Quaternary vents extends to the northern coast of the peninsula. Lysuholl is the central of three volcanic systems occupying the peninsula. The latest eruption from Lysuholl is undated, but the volcanic field has been active during the Holocene.</obo:IAO_0000115>
        <oboInOwl:hasOBONamespace>GAZ</oboInOwl:hasOBONamespace>
        <oboInOwl:id>GAZ:00051979</oboInOwl:id>
        <rdfs:label>Lysuholl Volcanic System</rdfs:label>
    </owl:NamedIndividual>
    


    <!-- http://purl.obolibrary.org/obo/GAZ_00051980 -->

    <owl:NamedIndividual rdf:about="http://purl.obolibrary.org/obo/GAZ_00051980">
        <obo:RO_0001025 rdf:resource="http://purl.obolibrary.org/obo/GAZ_00062086"/>
        <obo:IAO_0000115>A volcanic system eastern end of the Snaefellsnes Peninsula that is composed of a group of alkali olivine basaltic cinder cones and lava flows along short fissures on a roughly 90 km-long WNW-ESE line. The volcanic field is about 20 km wide at the eastern end and narrows to about 10 km width on the west. Youthful-looking cinder cones and lava flows with morphologically pristine surfaces testify to numerous eruptions during the Holocene. The latest eruption post-dated the settlement of Iceland, and took place about 1000 years ago.</obo:IAO_0000115>
        <oboInOwl:hasOBONamespace>GAZ</oboInOwl:hasOBONamespace>
        <oboInOwl:id>GAZ:00051980</oboInOwl:id>
        <rdfs:label>Ljosufjoll Volcanic System</rdfs:label>
    </owl:NamedIndividual>
    


    <!-- http://purl.obolibrary.org/obo/GAZ_00053296 -->

    <owl:NamedIndividual rdf:about="http://purl.obolibrary.org/obo/GAZ_00053296">
        <obo:RO_0001025 rdf:resource="http://purl.obolibrary.org/obo/GAZ_00001204"/>
        <obo:IAO_0000115>A stratovolcano located north of Myrdalsjokull and south of Thorisvatn lake, is cut by a 12 km wide caldera that formed during the Pleistocene. Torjajokull consists of the largest area of silicic and intermediate volcanism in Iceland; about 225 cu km of silicic extrusive rocks are exposed. The dominantly rhyolitic complex rises about 500m above surrounding basaltic plains and is elongated in a WNW-ESE direction. Most rhyolitic lava flows were erupted subglacially, forming silicic hyaloclastites that form ridge and dome-shaped breccias. During postglacial times only a narrow fissure zone at the western end has been active, producing mostly silicic lava flows, lava domes, and tephras.</obo:IAO_0000115>
        <oboInOwl:hasOBONamespace>GAZ</oboInOwl:hasOBONamespace>
        <oboInOwl:id>GAZ:00053296</oboInOwl:id>
        <rdfs:label>Torfajokull</rdfs:label>
    </owl:NamedIndividual>
    


    <!-- http://purl.obolibrary.org/obo/GAZ_00053297 -->

    <owl:NamedIndividual rdf:about="http://purl.obolibrary.org/obo/GAZ_00053297">
        <obo:RO_0001025 rdf:resource="http://purl.obolibrary.org/obo/GAZ_00001204"/>
        <obo:IAO_0000115>A glacially dissected, largely Pleistocene rhyolitic central volcano (stratovolcano) located SW of the Hofsjokull icecap. Steep-sided Pleistocene rhyolitic lava domes and numerous hot springs occupy two calderas at the center of the 5 x 7 km wide complex. Holocene flank fissures on the NE side produced the Illahraun lava flow, which traveled more than 20 km to the south. Fumarolic activity at Kerlingarfjoll, mostly concentrated in the center of the complex, is the most vigorous in Iceland.</obo:IAO_0000115>
        <oboInOwl:hasOBONamespace>GAZ</oboInOwl:hasOBONamespace>
        <oboInOwl:id>GAZ:00053297</oboInOwl:id>
        <rdfs:label>Kerlingarfjoll</rdfs:label>
    </owl:NamedIndividual>
    


    <!-- http://purl.obolibrary.org/obo/GAZ_00053298 -->

    <owl:NamedIndividual rdf:about="http://purl.obolibrary.org/obo/GAZ_00053298">
        <obo:RO_0001025 rdf:resource="http://purl.obolibrary.org/obo/GAZ_00001204"/>
        <obo:IAO_0000115>A volcanic system, located east of Kleifarvatn lake, consists of a series of NE-SW-trending crater rows and small shield volcanoes.</obo:IAO_0000115>
        <oboInOwl:hasOBONamespace>GAZ</oboInOwl:hasOBONamespace>
        <oboInOwl:id>GAZ:00053298</oboInOwl:id>
        <rdfs:label>Brennisteinsfjoll</rdfs:label>
    </owl:NamedIndividual>
    


    <!-- http://purl.obolibrary.org/obo/GAZ_00053299 -->

    <owl:NamedIndividual rdf:about="http://purl.obolibrary.org/obo/GAZ_00053299">
        <obo:RO_0001025 rdf:resource="http://purl.obolibrary.org/obo/GAZ_00053327"/>
        <obo:IAO_0000115>A subglacial volcano lies along an east-west-trending area connecting the two principal rift zones of Iceland. It bridges the gap between the Reykjanes-Langjokull rift on the west, which terminates at Langjokull, and the eastern zone, which extends NE-ward across east-central Iceland. The roughly 7 x 11 km central caldera of Hofsjokull volcano lies beneath the western part of the massive Hofsjokull icecap. A small Holocene shield volcano is located at the SW margin of the icecap.</obo:IAO_0000115>
        <oboInOwl:hasOBONamespace>GAZ</oboInOwl:hasOBONamespace>
        <oboInOwl:id>GAZ:00053299</oboInOwl:id>
        <rdfs:label>Hofsjokull Volcano</rdfs:label>
    </owl:NamedIndividual>
    


    <!-- http://purl.obolibrary.org/obo/GAZ_00053300 -->

    <owl:NamedIndividual rdf:about="http://purl.obolibrary.org/obo/GAZ_00053300">
        <obo:RO_0001025 rdf:resource="http://purl.obolibrary.org/obo/GAZ_00280523"/>
        <obo:IAO_0000115>A submarine volcanic system off the SW tip of Iceland is part of the Mid-Atlantic Ridge, which is exposed subaerially in Iceland.</obo:IAO_0000115>
        <oboInOwl:hasOBONamespace>GAZ</oboInOwl:hasOBONamespace>
        <oboInOwl:id>GAZ:00053300</oboInOwl:id>
        <rdfs:label>Reykjaneshryggur</rdfs:label>
    </owl:NamedIndividual>
    


    <!-- http://purl.obolibrary.org/obo/GAZ_00053301 -->

    <owl:NamedIndividual rdf:about="http://purl.obolibrary.org/obo/GAZ_00053301">
        <obo:RO_0001025 rdf:resource="http://purl.obolibrary.org/obo/GAZ_00001204"/>
        <obo:IAO_0000115>A stratovolcano that lies near the southern end of the eastern rift zone. Hekla occupies a rift-transform junction, and has produced basaltic andesites, in contrast to the tholeiitic basalts typical of Icelandic rift zone volcanoes. A 5.5 km-long fissure, Heklugja, cuts across the 1491 m high volcano and is often active along its full length during major eruptions. Repeated eruptions along this rift, which is oblique to most rifting structures in the eastern volcanic zone, are responsible for Hekla&apos;s elongated ENE-WSW profile.</obo:IAO_0000115>
        <oboInOwl:hasOBONamespace>GAZ</oboInOwl:hasOBONamespace>
        <oboInOwl:id>GAZ:00053301</oboInOwl:id>
        <rdfs:label>Hekla</rdfs:label>
    </owl:NamedIndividual>
    


    <!-- http://purl.obolibrary.org/obo/GAZ_00053302 -->

    <owl:NamedIndividual rdf:about="http://purl.obolibrary.org/obo/GAZ_00053302">
        <obo:RO_0001025 rdf:resource="http://purl.obolibrary.org/obo/GAZ_00001206"/>
        <obo:IAO_0000115>A subglacial volcano at the SW end of the Langjokull icecap has associated rift zones to the north and SW that have erupted during the Holocene. Hot springs are associated with the rhyolitic Prestahnukur central volcano.</obo:IAO_0000115>
        <oboInOwl:hasOBONamespace>GAZ</oboInOwl:hasOBONamespace>
        <oboInOwl:id>GAZ:00053302</oboInOwl:id>
        <rdfs:label>Prestahnukur</rdfs:label>
    </owl:NamedIndividual>
    


    <!-- http://purl.obolibrary.org/obo/GAZ_00053303 -->

    <owl:NamedIndividual rdf:about="http://purl.obolibrary.org/obo/GAZ_00053303">
        <obo:RO_0001025 rdf:resource="http://purl.obolibrary.org/obo/GAZ_00053326"/>
        <obo:IAO_0000115>A stratovolcano lies at the northern end of an active volcanic zone that extends to the NE from the Reykjanes Peninsula. Langjokull volcano occupies the NE half of the massive Langjokull icecap, east of the prominent Pleistocene table mountain, Erikskokull. A summit caldera lies beneath the ice. Several shield volcanoes have been constructed along flank fissure zones, and postglacial lava flows flank Langjokull on the northern, western, and eastern sides. One of the most prominent of these is a small shield volcano that was formed at the site of the massive Hallmundahraun lava flow, which covers 200 sq km, and was erupted shortly after 900 AD. The Geysir thermal area, containing Iceland&apos;s largest geysers, lies in the Haukadalur basin, near the southern end of the lengthy fissure system extending from Langjokull central volcano.</obo:IAO_0000115>
        <oboInOwl:hasOBONamespace>GAZ</oboInOwl:hasOBONamespace>
        <oboInOwl:id>GAZ:00053303</oboInOwl:id>
        <rdfs:label>Langjokull Volcano</rdfs:label>
    </owl:NamedIndividual>
    


    <!-- http://purl.obolibrary.org/obo/GAZ_00053305 -->

    <owl:NamedIndividual rdf:about="http://purl.obolibrary.org/obo/GAZ_00053305">
        <rdf:type rdf:resource="http://purl.obolibrary.org/obo/ENVO_00000354"/>
        <obo:RO_0001025 rdf:resource="http://purl.obolibrary.org/obo/GAZ_00008175"/>
        <obo:IAO_0000115>A volcanic system at the SW tip of the Reykjanes Peninsula, where the Mid Atlantic Ridge rises above sea level, comprises a broad area of postglacial basaltic crater rows and small shield volcanoes. The Reykjanes volcanic system is the westernmost of a series of four closely-spaced en-echelon fissure systems that extend diagonally across the Reykjanes Peninsula.</obo:IAO_0000115>
        <oboInOwl:hasOBONamespace>GAZ</oboInOwl:hasOBONamespace>
        <oboInOwl:id>GAZ:00053305</oboInOwl:id>
        <rdfs:label>Reykjanes</rdfs:label>
    </owl:NamedIndividual>
    


    <!-- http://purl.obolibrary.org/obo/GAZ_00053306 -->

    <owl:NamedIndividual rdf:about="http://purl.obolibrary.org/obo/GAZ_00053306">
        <obo:RO_0001025 rdf:resource="http://purl.obolibrary.org/obo/GAZ_00053328"/>
        <obo:IAO_0000115>A subglacial volcano located near the southern end of Iceland&apos;s eastern volcanic zone, is hidden beneath the Myrdalsjokull icecap. The subglacial basaltic-to-rhyolitic volcano is one of Iceland&apos;s most active and is a frequent producer of damaging jokulhlaups, or glacier-outburst floods. A large 9 x 14 km subglacial caldera with a long axis in a NW-SE direction is up to 750 m deep. Its high point reaches 1380 m, and three major outlet glaciers have breached its rim.</obo:IAO_0000115>
        <oboInOwl:hasOBONamespace>GAZ</oboInOwl:hasOBONamespace>
        <oboInOwl:id>GAZ:00053306</oboInOwl:id>
        <rdfs:label>Katla</rdfs:label>
    </owl:NamedIndividual>
    


    <!-- http://purl.obolibrary.org/obo/GAZ_00053307 -->

    <owl:NamedIndividual rdf:about="http://purl.obolibrary.org/obo/GAZ_00053307">
        <obo:RO_0001025 rdf:resource="http://purl.obolibrary.org/obo/GAZ_00053316"/>
        <obo:IAO_0000115>A system of fissure vents lying immediately SE of Hekla volcano; a 40 km-long, 9 km wide collection of alkali basaltic fissures and crater rows. Volcanism has migrated from the SW to the NE during the early to late Holocene. This volcanic system has been one of Iceland&apos;s most active.</obo:IAO_0000115>
        <oboInOwl:hasOBONamespace>GAZ</oboInOwl:hasOBONamespace>
        <oboInOwl:id>GAZ:00053307</oboInOwl:id>
        <rdfs:label>Vatnafjoll [volcano]</rdfs:label>
    </owl:NamedIndividual>
    


    <!-- http://purl.obolibrary.org/obo/GAZ_00053308 -->

    <owl:NamedIndividual rdf:about="http://purl.obolibrary.org/obo/GAZ_00053308">
        <obo:RO_0001025 rdf:resource="http://purl.obolibrary.org/obo/GAZ_00001204"/>
        <obo:IAO_0000115>A stratovolcano of the eastern volcanic zone of Iceland and has produced rocks of basaltic-to-rhyolitic composition.</obo:IAO_0000115>
        <oboInOwl:hasOBONamespace>GAZ</oboInOwl:hasOBONamespace>
        <oboInOwl:id>GAZ:00053308</oboInOwl:id>
        <rdfs:label>Tindfjallajokull</rdfs:label>
    </owl:NamedIndividual>
    


    <!-- http://purl.obolibrary.org/obo/GAZ_00053309 -->

    <owl:NamedIndividual rdf:about="http://purl.obolibrary.org/obo/GAZ_00053309">
        <obo:RO_0001025 rdf:resource="http://purl.obolibrary.org/obo/GAZ_00001204"/>
        <obo:IAO_0000115>A stratovolcano that consists of an E-W-trending, elongated ice-covered basaltic-andesite stratovolcano with a 2.5 km wide summit caldera. Fissure-fed lava flows occur on both the eastern and western flanks of the volcano, but are more prominent on the western side.</obo:IAO_0000115>
        <oboInOwl:hasOBONamespace>GAZ</oboInOwl:hasOBONamespace>
        <oboInOwl:id>GAZ:00053309</oboInOwl:id>
        <rdfs:label>Eyjafjoll</rdfs:label>
    </owl:NamedIndividual>
    


    <!-- http://purl.obolibrary.org/obo/GAZ_00053310 -->

    <owl:NamedIndividual rdf:about="http://purl.obolibrary.org/obo/GAZ_00053310">
        <obo:RO_0001025 rdf:resource="http://purl.obolibrary.org/obo/GAZ_00053316"/>
        <obo:IAO_0000115>A subglacial volcanic system is located immediately WNW of Grimsvotn volcano. Two subglacial ridges extend from the largely subglacial Hamarinn central volcano; the Loki ridge trends to the NE and the Fogrufjoll ridge to the SW.</obo:IAO_0000115>
        <oboInOwl:hasOBONamespace>GAZ</oboInOwl:hasOBONamespace>
        <oboInOwl:id>GAZ:00053310</oboInOwl:id>
        <rdfs:label>Loki-Fogrufjoll</rdfs:label>
    </owl:NamedIndividual>
    


    <!-- http://purl.obolibrary.org/obo/GAZ_00053311 -->

    <owl:NamedIndividual rdf:about="http://purl.obolibrary.org/obo/GAZ_00053311">
        <rdf:type rdf:resource="http://purl.obolibrary.org/obo/ENVO_00000354"/>
        <obo:RO_0001025 rdf:resource="http://purl.obolibrary.org/obo/GAZ_00001204"/>
        <obo:IAO_0000115>A volcanic system, cutting through Thingvallavatn lake, consists of a series of NE-SW-trending fissure vents, crater rows, and small shield volcanoes occupying a strongly faulted graben. Hengill is the easternmost of a series of four closely spaced basaltic fissure systems that cut diagonally across the Reykjanes Peninsula and lies at the triple junction of the Reykjanes Peninsula volcanic zone, the Western volcanic zone, and the South Iceland seismic zone.</obo:IAO_0000115>
        <oboInOwl:hasOBONamespace>GAZ</oboInOwl:hasOBONamespace>
        <oboInOwl:id>GAZ:00053311</oboInOwl:id>
        <rdfs:label>Hengill</rdfs:label>
    </owl:NamedIndividual>
    


    <!-- http://purl.obolibrary.org/obo/GAZ_00053312 -->

    <owl:NamedIndividual rdf:about="http://purl.obolibrary.org/obo/GAZ_00053312">
        <obo:RO_0001025 rdf:resource="http://purl.obolibrary.org/obo/GAZ_00280115"/>
        <obo:IAO_0000115>A stratovolcano located to the NW of the massive Vatnajokull icecap, contains two calderas. One is largely filled by the Tungnafellsjokull glacier, and the other ice-free caldera located to the SE contains Pleistocene rhyolitic lavas.</obo:IAO_0000115>
        <oboInOwl:hasOBONamespace>GAZ</oboInOwl:hasOBONamespace>
        <oboInOwl:id>GAZ:00053312</oboInOwl:id>
        <rdfs:label>Tungnafellsjokull [volcano]</rdfs:label>
    </owl:NamedIndividual>
    


    <!-- http://purl.obolibrary.org/obo/GAZ_00053313 -->

    <owl:NamedIndividual rdf:about="http://purl.obolibrary.org/obo/GAZ_00053313">
        <obo:RO_0001025 rdf:resource="http://purl.obolibrary.org/obo/GAZ_00001207"/>
        <obo:IAO_0000115>A subglacial stratovolcano that lies beneath the NW part of the Vatnajokull icecap, NW of Grimsvotn volcano, and contains a subglacial 700-m-deep caldera. Related fissure systems include the Veidivotn and Trollagigar fissures, which extend about 100 km SW to near Torfajokull volcano and 50 km NE to near Askja volcano, respectively.</obo:IAO_0000115>
        <oboInOwl:hasOBONamespace>GAZ</oboInOwl:hasOBONamespace>
        <oboInOwl:id>GAZ:00053313</oboInOwl:id>
        <rdfs:label>Bardarbunga</rdfs:label>
    </owl:NamedIndividual>
    


    <!-- http://purl.obolibrary.org/obo/GAZ_00053314 -->

    <owl:NamedIndividual rdf:about="http://purl.obolibrary.org/obo/GAZ_00053314">
        <rdf:type rdf:resource="http://purl.obolibrary.org/obo/ENVO_00000354"/>
        <obo:RO_0001025 rdf:resource="http://purl.obolibrary.org/obo/GAZ_00008175"/>
        <obo:IAO_0000115>A small volcanic system located SE of Thingvallavatn lake east of an en echelon group of volcanic fields extending across the Reykjanes Peninsula. Grimsnes lava flows cover 54 km2 and were erupted from a group of 11 fissures that produced a series of NE-SW-trending crater rows.</obo:IAO_0000115>
        <oboInOwl:hasOBONamespace>GAZ</oboInOwl:hasOBONamespace>
        <oboInOwl:id>GAZ:00053314</oboInOwl:id>
        <rdfs:label>Grimsnes</rdfs:label>
    </owl:NamedIndividual>
    


    <!-- http://purl.obolibrary.org/obo/GAZ_00053315 -->

    <owl:NamedIndividual rdf:about="http://purl.obolibrary.org/obo/GAZ_00053315">
        <obo:RO_0001025 rdf:resource="http://purl.obolibrary.org/obo/GAZ_00053316"/>
        <obo:IAO_0000115>A subglacial caldera that lies largely beneath the vast Vatnajokull icecap. The caldera lake is covered by a 200-m-thick ice shelf, and only the southern rim of the 6 x 8 km caldera is exposed. The geothermal area in the caldera causes frequent jokulhlaups (glacier outburst floods) when melting raises the water level high enough to lift its ice dam. Long NE-SW-trending fissure systems extend from the central volcano. The most prominent of these is the noted Laki (Skaftar) fissure, which extends to the SW and produced the world&apos;s largest known historical lava flow during an eruption in 1783.</obo:IAO_0000115>
        <oboInOwl:hasOBONamespace>GAZ</oboInOwl:hasOBONamespace>
        <oboInOwl:id>GAZ:00053315</oboInOwl:id>
        <rdfs:label>Grimsvotn [caldera]</rdfs:label>
    </owl:NamedIndividual>
    


    <!-- http://purl.obolibrary.org/obo/GAZ_00053316 -->

    <owl:NamedIndividual rdf:about="http://purl.obolibrary.org/obo/GAZ_00053316">
        <obo:IAO_0000115>A large glacier (icecap) in Iceland. It is located in the south-east of the island, covering more than 8% of the country.</obo:IAO_0000115>
        <oboInOwl:hasOBONamespace>GAZ</oboInOwl:hasOBONamespace>
        <oboInOwl:id>GAZ:00053316</oboInOwl:id>
        <rdfs:label>Vatnajokull</rdfs:label>
    </owl:NamedIndividual>
    


    <!-- http://purl.obolibrary.org/obo/GAZ_00053317 -->

    <owl:NamedIndividual rdf:about="http://purl.obolibrary.org/obo/GAZ_00053317">
        <obo:RO_0001025 rdf:resource="http://purl.obolibrary.org/obo/GAZ_00053316"/>
        <obo:IAO_0000115>A large subglacial stratovolcano at the NE end of the Vatnajokull icecap. Two elliptical ice-filled calderas, 8 x 5 km in diameter, have been identified. An associated fissure swarm can be traced 60 km to the NE. A half dozen ridges of subglacially erupted pillow lavas are now exposed and extend beyond the glacial icecap to the NE.</obo:IAO_0000115>
        <oboInOwl:hasOBONamespace>GAZ</oboInOwl:hasOBONamespace>
        <oboInOwl:id>GAZ:00053317</oboInOwl:id>
        <rdfs:label>Kverkfjoll</rdfs:label>
    </owl:NamedIndividual>
    


    <!-- http://purl.obolibrary.org/obo/GAZ_00053318 -->

    <owl:NamedIndividual rdf:about="http://purl.obolibrary.org/obo/GAZ_00053318">
        <obo:RO_0001025 rdf:resource="http://purl.obolibrary.org/obo/GAZ_00001203"/>
        <obo:IAO_0000115>A large basaltic central stratovolcano that forms the Dyngjufjoll massif. It is truncated by three overlapping calderas, the largest of which is 8 km wide and may have been produced primarily from subglacial ring-fracture eruptions rather than by subsidence.</obo:IAO_0000115>
        <oboInOwl:hasOBONamespace>GAZ</oboInOwl:hasOBONamespace>
        <oboInOwl:id>GAZ:00053318</oboInOwl:id>
        <rdfs:label>Askja</rdfs:label>
    </owl:NamedIndividual>
    


    <!-- http://purl.obolibrary.org/obo/GAZ_00053319 -->

    <owl:NamedIndividual rdf:about="http://purl.obolibrary.org/obo/GAZ_00053319">
        <obo:RO_0001025 rdf:resource="http://purl.obolibrary.org/obo/GAZ_00001207"/>
        <obo:IAO_0000115>A caldera located NE of Myvatn lake, is a topographically indistinct 10 km wide caldera that is cut by a N-S-trending fissure system. Eruption of a rhyolitic welded tuff about 100,000 years ago was associated with formation of the caldera.</obo:IAO_0000115>
        <oboInOwl:hasOBONamespace>GAZ</oboInOwl:hasOBONamespace>
        <oboInOwl:id>GAZ:00053319</oboInOwl:id>
        <rdfs:label>Krafla</rdfs:label>
    </owl:NamedIndividual>
    


    <!-- http://purl.obolibrary.org/obo/GAZ_00053320 -->

    <owl:NamedIndividual rdf:about="http://purl.obolibrary.org/obo/GAZ_00053320">
        <obo:RO_0001025 rdf:resource="http://purl.obolibrary.org/obo/GAZ_00001207"/>
        <obo:IAO_0000115>A stratovolcano NNE of Askja and SE of Myvatn lake, is a volcanic system that is being constructed over the basaltic Ketildyngja shield volcano. Associated fissure systems, including the Sveinar fissure, extend 130 km to the northern coast of Iceland. The Kerlingardyngja shield volcano to the south is also part of the Fremrinamur volcanic system.</obo:IAO_0000115>
        <oboInOwl:hasOBONamespace>GAZ</oboInOwl:hasOBONamespace>
        <oboInOwl:id>GAZ:00053320</oboInOwl:id>
        <rdfs:label>Fremrinamur</rdfs:label>
    </owl:NamedIndividual>
    


    <!-- http://purl.obolibrary.org/obo/GAZ_00053321 -->

    <owl:NamedIndividual rdf:about="http://purl.obolibrary.org/obo/GAZ_00053321">
        <obo:RO_0001025 rdf:resource="http://purl.obolibrary.org/obo/GAZ_00280522"/>
        <obo:IAO_0000115>A submarine volcano forming an oblique transform zone that separates the northern volcanic zone of Iceland from the Kolbeinsey Ridge, part of the Mid-Atlantic Ridge north of Iceland.</obo:IAO_0000115>
        <oboInOwl:hasOBONamespace>GAZ</oboInOwl:hasOBONamespace>
        <oboInOwl:id>GAZ:00053321</oboInOwl:id>
        <rdfs:label>Tjornes Fracture Zone</rdfs:label>
    </owl:NamedIndividual>
    


    <!-- http://purl.obolibrary.org/obo/GAZ_00053322 -->

    <owl:NamedIndividual rdf:about="http://purl.obolibrary.org/obo/GAZ_00053322">
        <obo:RO_0001025 rdf:resource="http://purl.obolibrary.org/obo/GAZ_00053316"/>
        <obo:IAO_0000115>A subglacial volcano at the SE part of the Vatnajokull icecap, north of Oroefajokull volcano, may contain a central caldera.</obo:IAO_0000115>
        <oboInOwl:hasOBONamespace>GAZ</oboInOwl:hasOBONamespace>
        <oboInOwl:id>GAZ:00053322</oboInOwl:id>
        <rdfs:label>Esjufjoll</rdfs:label>
    </owl:NamedIndividual>
    


    <!-- http://purl.obolibrary.org/obo/GAZ_00053323 -->

    <owl:NamedIndividual rdf:about="http://purl.obolibrary.org/obo/GAZ_00053323">
        <obo:RO_0001025 rdf:resource="http://purl.obolibrary.org/obo/GAZ_00053316"/>
        <obo:IAO_0000115>A broad glacier-clad central stratovolcano at the SE end of the Vatnajokull icecap. A 4 x 5 km subglacial caldera truncates the summit of the dominantly basaltic and rhyolitic volcano. The extensive summit icecap is drained through deep glacial valleys dissecting the SW-to-SE flanks of the volcano.</obo:IAO_0000115>
        <oboInOwl:hasOBONamespace>GAZ</oboInOwl:hasOBONamespace>
        <oboInOwl:id>GAZ:00053323</oboInOwl:id>
        <rdfs:label>Oraefajokull</rdfs:label>
    </owl:NamedIndividual>
    


    <!-- http://purl.obolibrary.org/obo/GAZ_00053324 -->

    <owl:NamedIndividual rdf:about="http://purl.obolibrary.org/obo/GAZ_00053324">
        <obo:RO_0001025 rdf:resource="http://purl.obolibrary.org/obo/GAZ_00001207"/>
        <obo:IAO_0000115>A basaltic shield volcano and its associated N-S fissure system extends from north of Myvatn lake to the northern coast of Iceland. The low, 564 m high Theistareykjarbunga shield volcano is the northernmost subaerial volcanic system along the eastern volcanic zone of Iceland.</obo:IAO_0000115>
        <oboInOwl:hasOBONamespace>GAZ</oboInOwl:hasOBONamespace>
        <oboInOwl:id>GAZ:00053324</oboInOwl:id>
        <rdfs:label>Theistareykjarbunga</rdfs:label>
    </owl:NamedIndividual>
    


    <!-- http://purl.obolibrary.org/obo/GAZ_00053326 -->

    <owl:NamedIndividual rdf:about="http://purl.obolibrary.org/obo/GAZ_00053326">
        <obo:RO_0001025 rdf:resource="http://purl.obolibrary.org/obo/GAZ_00001206"/>
        <obo:IAO_0000115>The second-largest of the glaciers of Iceland (1.021 km2). It is situated in the west of the Icelandic Interior or Highlands of Iceland.</obo:IAO_0000115>
        <oboInOwl:hasOBONamespace>GAZ</oboInOwl:hasOBONamespace>
        <oboInOwl:id>GAZ:00053326</oboInOwl:id>
        <rdfs:label>Langjokull</rdfs:label>
    </owl:NamedIndividual>
    


    <!-- http://purl.obolibrary.org/obo/GAZ_00053327 -->

    <owl:NamedIndividual rdf:about="http://purl.obolibrary.org/obo/GAZ_00053327">
        <obo:RO_0001025 rdf:resource="http://purl.obolibrary.org/obo/GAZ_00001202"/>
        <obo:IAO_0000115>A glacier (icecap) covering an area of 925 km2. Its highest peak reaches 1,765 m. It is situated in the west of the Icelandic Interior or Highlands of Iceland between Vatnajokull and Langjokull. Hofsjokull is the source of several rivers including the Pjorsa Iceland&apos;s longest river.</obo:IAO_0000115>
        <oboInOwl:hasOBONamespace>GAZ</oboInOwl:hasOBONamespace>
        <oboInOwl:id>GAZ:00053327</oboInOwl:id>
        <rdfs:label>Hofsjokull</rdfs:label>
    </owl:NamedIndividual>
    


    <!-- http://purl.obolibrary.org/obo/GAZ_00053328 -->

    <owl:NamedIndividual rdf:about="http://purl.obolibrary.org/obo/GAZ_00053328">
        <obo:RO_0001025 rdf:resource="http://purl.obolibrary.org/obo/GAZ_00001204"/>
        <obo:IAO_0000115>An ice cap. A glacier in the south of Iceland. It is situated to the north of Vik i Myrdal and to the east of the smaller glacier Eyjafjallajokull.</obo:IAO_0000115>
        <oboInOwl:hasOBONamespace>GAZ</oboInOwl:hasOBONamespace>
        <oboInOwl:id>GAZ:00053328</oboInOwl:id>
        <rdfs:label>Myrdalsjokull</rdfs:label>
    </owl:NamedIndividual>
    


    <!-- http://purl.obolibrary.org/obo/GAZ_00053329 -->

    <owl:NamedIndividual rdf:about="http://purl.obolibrary.org/obo/GAZ_00053329">
        <obo:RO_0001025 rdf:resource="http://purl.obolibrary.org/obo/GAZ_00145765"/>
        <obo:IAO_0000115>The northernmost glacier of Iceland. It is situated south-west of the peninsula Hornstrandir in the Vestfirdir region.</obo:IAO_0000115>
        <oboInOwl:hasOBONamespace>GAZ</oboInOwl:hasOBONamespace>
        <oboInOwl:id>GAZ:00053329</oboInOwl:id>
        <rdfs:label>Drangajokull</rdfs:label>
    </owl:NamedIndividual>
    


    <!-- http://purl.obolibrary.org/obo/GAZ_00053330 -->

    <owl:NamedIndividual rdf:about="http://purl.obolibrary.org/obo/GAZ_00053330">
        <obo:RO_0001025 rdf:resource="http://purl.obolibrary.org/obo/GAZ_00001204"/>
        <obo:IAO_0000115>A glacier of Iceland. It is situated to the north of Skogar and to the west of the larger glacier Myrdalsjokull.</obo:IAO_0000115>
        <oboInOwl:hasOBONamespace>GAZ</oboInOwl:hasOBONamespace>
        <oboInOwl:id>GAZ:00053330</oboInOwl:id>
        <rdfs:label>Eyjafjallajokull [ice cap]</rdfs:label>
    </owl:NamedIndividual>
    


    <!-- http://purl.obolibrary.org/obo/GAZ_00053331 -->

    <owl:NamedIndividual rdf:about="http://purl.obolibrary.org/obo/GAZ_00053331">
        <obo:RO_0001025 rdf:resource="http://purl.obolibrary.org/obo/GAZ_00051978"/>
        <obo:IAO_0000115>A glacier (icecap) covering the Snaefellsokull volcano. It is situated on the most western part of the Snoefellsnes peninsula in Iceland.</obo:IAO_0000115>
        <oboInOwl:hasOBONamespace>GAZ</oboInOwl:hasOBONamespace>
        <oboInOwl:id>GAZ:00053331</oboInOwl:id>
        <rdfs:label>Snaefellsjokull [icecap]</rdfs:label>
    </owl:NamedIndividual>
    


    <!-- http://purl.obolibrary.org/obo/GAZ_00053332 -->

    <owl:NamedIndividual rdf:about="http://purl.obolibrary.org/obo/GAZ_00053332">
        <obo:RO_0001025 rdf:resource="http://purl.obolibrary.org/obo/GAZ_00020031"/>
        <obo:RO_0001025 rdf:resource="http://purl.obolibrary.org/obo/GAZ_00280522"/>
        <obo:IAO_0000115>A fjord in Northern Iceland, situated between Trollaskagi and Skagi.</obo:IAO_0000115>
        <oboInOwl:hasOBONamespace>GAZ</oboInOwl:hasOBONamespace>
        <oboInOwl:id>GAZ:00053332</oboInOwl:id>
        <rdfs:label>Skagafjoerdur</rdfs:label>
    </owl:NamedIndividual>
    


    <!-- http://purl.obolibrary.org/obo/GAZ_00053333 -->

    <owl:NamedIndividual rdf:about="http://purl.obolibrary.org/obo/GAZ_00053333">
        <obo:RO_0001025 rdf:resource="http://purl.obolibrary.org/obo/GAZ_00001206"/>
        <obo:RO_0001025 rdf:resource="http://purl.obolibrary.org/obo/GAZ_00280523"/>
        <obo:IAO_0000115>A large shallow bay, about 50 km wide and 125 km long and located in the west of Iceland. It separates the region of the West Fjords from the rest of the country.</obo:IAO_0000115>
        <oboInOwl:hasOBONamespace>GAZ</oboInOwl:hasOBONamespace>
        <oboInOwl:id>GAZ:00053333</oboInOwl:id>
        <rdfs:label>Breidafjoerdur</rdfs:label>
    </owl:NamedIndividual>
    


    <!-- http://purl.obolibrary.org/obo/GAZ_00053334 -->

    <owl:NamedIndividual rdf:about="http://purl.obolibrary.org/obo/GAZ_00053334">
        <obo:RO_0001025 rdf:resource="http://purl.obolibrary.org/obo/GAZ_00053333"/>
        <obo:IAO_0000115>An island in Breidhafjrdhur.</obo:IAO_0000115>
        <oboInOwl:hasOBONamespace>GAZ</oboInOwl:hasOBONamespace>
        <oboInOwl:id>GAZ:00053334</oboInOwl:id>
        <rdfs:label>Hergilsey</rdfs:label>
    </owl:NamedIndividual>
    


    <!-- http://purl.obolibrary.org/obo/GAZ_00053335 -->

    <owl:NamedIndividual rdf:about="http://purl.obolibrary.org/obo/GAZ_00053335">
        <obo:RO_0001025 rdf:resource="http://purl.obolibrary.org/obo/GAZ_00053333"/>
        <obo:IAO_0000115>An island in Breidhafjrdhur.</obo:IAO_0000115>
        <oboInOwl:hasOBONamespace>GAZ</oboInOwl:hasOBONamespace>
        <oboInOwl:id>GAZ:00053335</oboInOwl:id>
        <rdfs:label>Skaleyjar</rdfs:label>
    </owl:NamedIndividual>
    


    <!-- http://purl.obolibrary.org/obo/GAZ_00053336 -->

    <owl:NamedIndividual rdf:about="http://purl.obolibrary.org/obo/GAZ_00053336">
        <obo:RO_0001025 rdf:resource="http://purl.obolibrary.org/obo/GAZ_00053333"/>
        <obo:IAO_0000115>An island in Breidhafjrdhur.</obo:IAO_0000115>
        <oboInOwl:hasOBONamespace>GAZ</oboInOwl:hasOBONamespace>
        <oboInOwl:id>GAZ:00053336</oboInOwl:id>
        <rdfs:label>Svidnur</rdfs:label>
    </owl:NamedIndividual>
    


    <!-- http://purl.obolibrary.org/obo/GAZ_00053337 -->

    <owl:NamedIndividual rdf:about="http://purl.obolibrary.org/obo/GAZ_00053337">
        <obo:RO_0001025 rdf:resource="http://purl.obolibrary.org/obo/GAZ_00053333"/>
        <obo:IAO_0000115>An island in Breidhafjrdhur.</obo:IAO_0000115>
        <oboInOwl:hasOBONamespace>GAZ</oboInOwl:hasOBONamespace>
        <oboInOwl:id>GAZ:00053337</oboInOwl:id>
        <rdfs:label>Hvallatur</rdfs:label>
    </owl:NamedIndividual>
    


    <!-- http://purl.obolibrary.org/obo/GAZ_00053338 -->

    <owl:NamedIndividual rdf:about="http://purl.obolibrary.org/obo/GAZ_00053338">
        <obo:RO_0001025 rdf:resource="http://purl.obolibrary.org/obo/GAZ_00053333"/>
        <obo:IAO_0000115>An island in Breidhafjrdhur.</obo:IAO_0000115>
        <oboInOwl:hasOBONamespace>GAZ</oboInOwl:hasOBONamespace>
        <oboInOwl:id>GAZ:00053338</oboInOwl:id>
        <rdfs:label>Svefneyjar</rdfs:label>
    </owl:NamedIndividual>
    


    <!-- http://purl.obolibrary.org/obo/GAZ_00053339 -->

    <owl:NamedIndividual rdf:about="http://purl.obolibrary.org/obo/GAZ_00053339">
        <obo:RO_0001025 rdf:resource="http://purl.obolibrary.org/obo/GAZ_00001207"/>
        <obo:RO_0001025 rdf:resource="http://purl.obolibrary.org/obo/GAZ_00280522"/>
        <obo:IAO_0000115>A bay in N Iceland. Originally created by glacial activity, has two major streams flowing into it: Skjalfandafljot, which is a glacier river and Laxa, which is a freshwater river.</obo:IAO_0000115>
        <oboInOwl:hasOBONamespace>GAZ</oboInOwl:hasOBONamespace>
        <oboInOwl:id>GAZ:00053339</oboInOwl:id>
        <rdfs:label>Skjalfandi</rdfs:label>
    </owl:NamedIndividual>
    


    <!-- http://purl.obolibrary.org/obo/GAZ_00053340 -->

    <owl:NamedIndividual rdf:about="http://purl.obolibrary.org/obo/GAZ_00053340">
        <obo:RO_0001025 rdf:resource="http://purl.obolibrary.org/obo/GAZ_00008739"/>
        <oboInOwl:hasOBONamespace>GAZ</oboInOwl:hasOBONamespace>
        <oboInOwl:id>GAZ:00053340</oboInOwl:id>
        <rdfs:label>Smaeyjar</rdfs:label>
    </owl:NamedIndividual>
    


    <!-- http://purl.obolibrary.org/obo/GAZ_00053341 -->

    <owl:NamedIndividual rdf:about="http://purl.obolibrary.org/obo/GAZ_00053341">
        <obo:RO_0001025 rdf:resource="http://purl.obolibrary.org/obo/GAZ_00053340"/>
        <obo:IAO_0000115>An island.</obo:IAO_0000115>
        <oboInOwl:hasOBONamespace>GAZ</oboInOwl:hasOBONamespace>
        <oboInOwl:id>GAZ:00053341</oboInOwl:id>
        <rdfs:label>Hrauney</rdfs:label>
    </owl:NamedIndividual>
    


    <!-- http://purl.obolibrary.org/obo/GAZ_00053342 -->

    <owl:NamedIndividual rdf:about="http://purl.obolibrary.org/obo/GAZ_00053342">
        <obo:RO_0001025 rdf:resource="http://purl.obolibrary.org/obo/GAZ_00053340"/>
        <obo:IAO_0000115>An island.</obo:IAO_0000115>
        <oboInOwl:hasOBONamespace>GAZ</oboInOwl:hasOBONamespace>
        <oboInOwl:id>GAZ:00053342</oboInOwl:id>
        <rdfs:label>Hani</rdfs:label>
    </owl:NamedIndividual>
    


    <!-- http://purl.obolibrary.org/obo/GAZ_00053343 -->

    <owl:NamedIndividual rdf:about="http://purl.obolibrary.org/obo/GAZ_00053343">
        <obo:RO_0001025 rdf:resource="http://purl.obolibrary.org/obo/GAZ_00053340"/>
        <obo:IAO_0000115>A skerry.</obo:IAO_0000115>
        <oboInOwl:hasOBONamespace>GAZ</oboInOwl:hasOBONamespace>
        <oboInOwl:id>GAZ:00053343</oboInOwl:id>
        <rdfs:label>Grasleysa</rdfs:label>
    </owl:NamedIndividual>
    


    <!-- http://purl.obolibrary.org/obo/GAZ_00053344 -->

    <owl:NamedIndividual rdf:about="http://purl.obolibrary.org/obo/GAZ_00053344">
        <obo:RO_0001025 rdf:resource="http://purl.obolibrary.org/obo/GAZ_00053340"/>
        <obo:IAO_0000115>An island.</obo:IAO_0000115>
        <oboInOwl:hasOBONamespace>GAZ</oboInOwl:hasOBONamespace>
        <oboInOwl:id>GAZ:00053344</oboInOwl:id>
        <rdfs:label>Haena</rdfs:label>
    </owl:NamedIndividual>
    


    <!-- http://purl.obolibrary.org/obo/GAZ_00053345 -->

    <owl:NamedIndividual rdf:about="http://purl.obolibrary.org/obo/GAZ_00053345">
        <obo:RO_0001025 rdf:resource="http://purl.obolibrary.org/obo/GAZ_00008739"/>
        <obo:IAO_0000115>An island.</obo:IAO_0000115>
        <oboInOwl:hasOBONamespace>GAZ</oboInOwl:hasOBONamespace>
        <oboInOwl:id>GAZ:00053345</oboInOwl:id>
        <rdfs:label>Geirfuglasker</rdfs:label>
    </owl:NamedIndividual>
    


    <!-- http://purl.obolibrary.org/obo/GAZ_00053346 -->

    <owl:NamedIndividual rdf:about="http://purl.obolibrary.org/obo/GAZ_00053346">
        <obo:RO_0001025 rdf:resource="http://purl.obolibrary.org/obo/GAZ_00008739"/>
        <obo:IAO_0000115>An island.</obo:IAO_0000115>
        <oboInOwl:hasOBONamespace>GAZ</oboInOwl:hasOBONamespace>
        <oboInOwl:id>GAZ:00053346</oboInOwl:id>
        <rdfs:label>Sudurey</rdfs:label>
    </owl:NamedIndividual>
    


    <!-- http://purl.obolibrary.org/obo/GAZ_00053347 -->

    <owl:NamedIndividual rdf:about="http://purl.obolibrary.org/obo/GAZ_00053347">
        <obo:RO_0001025 rdf:resource="http://purl.obolibrary.org/obo/GAZ_00008739"/>
        <obo:IAO_0000115>An island.</obo:IAO_0000115>
        <oboInOwl:hasOBONamespace>GAZ</oboInOwl:hasOBONamespace>
        <oboInOwl:id>GAZ:00053347</oboInOwl:id>
        <rdfs:label>Sulnasker</rdfs:label>
    </owl:NamedIndividual>
    


    <!-- http://purl.obolibrary.org/obo/GAZ_00053348 -->

    <owl:NamedIndividual rdf:about="http://purl.obolibrary.org/obo/GAZ_00053348">
        <obo:RO_0001025 rdf:resource="http://purl.obolibrary.org/obo/GAZ_00008739"/>
        <obo:IAO_0000115>An island.</obo:IAO_0000115>
        <oboInOwl:hasOBONamespace>GAZ</oboInOwl:hasOBONamespace>
        <oboInOwl:id>GAZ:00053348</oboInOwl:id>
        <rdfs:label>Hellisey</rdfs:label>
    </owl:NamedIndividual>
    


    <!-- http://purl.obolibrary.org/obo/GAZ_00053349 -->

    <owl:NamedIndividual rdf:about="http://purl.obolibrary.org/obo/GAZ_00053349">
        <obo:RO_0001025 rdf:resource="http://purl.obolibrary.org/obo/GAZ_00008739"/>
        <obo:IAO_0000115>An island.</obo:IAO_0000115>
        <oboInOwl:hasOBONamespace>GAZ</oboInOwl:hasOBONamespace>
        <oboInOwl:id>GAZ:00053349</oboInOwl:id>
        <rdfs:label>Geldungur</rdfs:label>
    </owl:NamedIndividual>
    


    <!-- http://purl.obolibrary.org/obo/GAZ_00053350 -->

    <owl:NamedIndividual rdf:about="http://purl.obolibrary.org/obo/GAZ_00053350">
        <obo:RO_0001025 rdf:resource="http://purl.obolibrary.org/obo/GAZ_00008739"/>
        <obo:IAO_0000115>An island.</obo:IAO_0000115>
        <oboInOwl:hasOBONamespace>GAZ</oboInOwl:hasOBONamespace>
        <oboInOwl:id>GAZ:00053350</oboInOwl:id>
        <rdfs:label>Ellidaey</rdfs:label>
    </owl:NamedIndividual>
    


    <!-- http://purl.obolibrary.org/obo/GAZ_00053351 -->

    <owl:NamedIndividual rdf:about="http://purl.obolibrary.org/obo/GAZ_00053351">
        <obo:RO_0001025 rdf:resource="http://purl.obolibrary.org/obo/GAZ_00008739"/>
        <obo:IAO_0000115>An island.</obo:IAO_0000115>
        <oboInOwl:hasOBONamespace>GAZ</oboInOwl:hasOBONamespace>
        <oboInOwl:id>GAZ:00053351</oboInOwl:id>
        <rdfs:label>Alsey</rdfs:label>
    </owl:NamedIndividual>
    


    <!-- http://purl.obolibrary.org/obo/GAZ_00053352 -->

    <owl:NamedIndividual rdf:about="http://purl.obolibrary.org/obo/GAZ_00053352">
        <obo:RO_0001025 rdf:resource="http://purl.obolibrary.org/obo/GAZ_00008739"/>
        <obo:IAO_0000115>An island.</obo:IAO_0000115>
        <oboInOwl:hasOBONamespace>GAZ</oboInOwl:hasOBONamespace>
        <oboInOwl:id>GAZ:00053352</oboInOwl:id>
        <rdfs:label>Bjarnarey</rdfs:label>
    </owl:NamedIndividual>
    


    <!-- http://purl.obolibrary.org/obo/GAZ_00053353 -->

    <owl:NamedIndividual rdf:about="http://purl.obolibrary.org/obo/GAZ_00053353">
        <obo:RO_0001025 rdf:resource="http://purl.obolibrary.org/obo/GAZ_00008739"/>
        <obo:IAO_0000115>An island.</obo:IAO_0000115>
        <oboInOwl:hasOBONamespace>GAZ</oboInOwl:hasOBONamespace>
        <oboInOwl:id>GAZ:00053353</oboInOwl:id>
        <rdfs:label>Brandur</rdfs:label>
    </owl:NamedIndividual>
    


    <!-- http://purl.obolibrary.org/obo/GAZ_00053354 -->

    <owl:NamedIndividual rdf:about="http://purl.obolibrary.org/obo/GAZ_00053354">
        <obo:RO_0001025 rdf:resource="http://purl.obolibrary.org/obo/GAZ_00280522"/>
        <obo:IAO_0000115>The longest fjord in central northern Iceland.</obo:IAO_0000115>
        <oboInOwl:hasOBONamespace>GAZ</oboInOwl:hasOBONamespace>
        <oboInOwl:id>GAZ:00053354</oboInOwl:id>
        <rdfs:label>Eyjafjoerdur</rdfs:label>
    </owl:NamedIndividual>
    


    <!-- http://purl.obolibrary.org/obo/GAZ_00059062 -->

    <owl:NamedIndividual rdf:about="http://purl.obolibrary.org/obo/GAZ_00059062">
        <obo:RO_0001025 rdf:resource="http://purl.obolibrary.org/obo/GAZ_00059063"/>
        <obo:IAO_0000115>A monomictic lake in the south-west of Iceland.</obo:IAO_0000115>
        <oboInOwl:hasOBONamespace>GAZ</oboInOwl:hasOBONamespace>
        <oboInOwl:id>GAZ:00059062</oboInOwl:id>
        <rdfs:label>Thingvallavatn</rdfs:label>
    </owl:NamedIndividual>
    


    <!-- http://purl.obolibrary.org/obo/GAZ_00059063 -->

    <owl:NamedIndividual rdf:about="http://purl.obolibrary.org/obo/GAZ_00059063">
        <obo:RO_0001025 rdf:resource="http://purl.obolibrary.org/obo/GAZ_00001204"/>
        <obo:IAO_0000115>A national park (since 1928) in the SW of Iceland near the peninsula of Reykjanes and the Hengill volcanic area.</obo:IAO_0000115>
        <oboInOwl:hasOBONamespace>GAZ</oboInOwl:hasOBONamespace>
        <oboInOwl:id>GAZ:00059063</oboInOwl:id>
        <rdfs:label>Thingvellir National Park</rdfs:label>
    </owl:NamedIndividual>
    


    <!-- http://purl.obolibrary.org/obo/GAZ_00062053 -->

    <owl:NamedIndividual rdf:about="http://purl.obolibrary.org/obo/GAZ_00062053">
        <obo:RO_0001025 rdf:resource="http://purl.obolibrary.org/obo/GAZ_00001204"/>
        <obo:IAO_0000115>A lake in southwest Iceland.</obo:IAO_0000115>
        <oboInOwl:hasOBONamespace>GAZ</oboInOwl:hasOBONamespace>
        <oboInOwl:id>GAZ:00062053</oboInOwl:id>
        <rdfs:label>Apavatn</rdfs:label>
    </owl:NamedIndividual>
    


    <!-- http://purl.obolibrary.org/obo/GAZ_00062054 -->

    <owl:NamedIndividual rdf:about="http://purl.obolibrary.org/obo/GAZ_00062054">
        <obo:RO_0001025 rdf:resource="http://purl.obolibrary.org/obo/GAZ_00001202"/>
        <obo:IAO_0000115>A reservoir. It was created in 1984-1991 as a reservoir for the Blonduvirkjun power plant.</obo:IAO_0000115>
        <oboInOwl:hasOBONamespace>GAZ</oboInOwl:hasOBONamespace>
        <oboInOwl:id>GAZ:00062054</oboInOwl:id>
        <rdfs:label>Blondulon</rdfs:label>
    </owl:NamedIndividual>
    


    <!-- http://purl.obolibrary.org/obo/GAZ_00062055 -->

    <owl:NamedIndividual rdf:about="http://purl.obolibrary.org/obo/GAZ_00062055">
        <obo:RO_0001025 rdf:resource="http://purl.obolibrary.org/obo/GAZ_00001203"/>
        <obo:IAO_0000115>A glacier lake at the south end of the Icelandic glacier Vatnajokull.</obo:IAO_0000115>
        <oboInOwl:hasOBONamespace>GAZ</oboInOwl:hasOBONamespace>
        <oboInOwl:id>GAZ:00062055</oboInOwl:id>
        <rdfs:label>Breidarlon</rdfs:label>
    </owl:NamedIndividual>
    


    <!-- http://purl.obolibrary.org/obo/GAZ_00062056 -->

    <owl:NamedIndividual rdf:about="http://purl.obolibrary.org/obo/GAZ_00062056">
        <obo:RO_0001025 rdf:resource="http://purl.obolibrary.org/obo/GAZ_00001203"/>
        <obo:IAO_0000115>A national park situated between Kirkjubaejarklaustur, typically referred to as Klaustur, and Hofn in the south of Iceland. Established 1967-09-15, and enlarged twice afterwards.</obo:IAO_0000115>
        <oboInOwl:hasOBONamespace>GAZ</oboInOwl:hasOBONamespace>
        <oboInOwl:id>GAZ:00062056</oboInOwl:id>
        <rdfs:label>Skaftafell National Park</rdfs:label>
    </owl:NamedIndividual>
    


    <!-- http://purl.obolibrary.org/obo/GAZ_00062057 -->

    <owl:NamedIndividual rdf:about="http://purl.obolibrary.org/obo/GAZ_00062057">
        <obo:RO_0001025 rdf:resource="http://purl.obolibrary.org/obo/GAZ_02000603"/>
        <obo:IAO_0000115>A lake in Iceland. It is situated in the area of Reykjavik.</obo:IAO_0000115>
        <oboInOwl:hasOBONamespace>GAZ</oboInOwl:hasOBONamespace>
        <oboInOwl:id>GAZ:00062057</oboInOwl:id>
        <rdfs:label>Ellidavatn</rdfs:label>
    </owl:NamedIndividual>
    


    <!-- http://purl.obolibrary.org/obo/GAZ_00062058 -->

    <owl:NamedIndividual rdf:about="http://purl.obolibrary.org/obo/GAZ_00062058">
        <obo:RO_0001025 rdf:resource="http://purl.obolibrary.org/obo/GAZ_00001203"/>
        <obo:IAO_0000115>A glacier lake at the south end of the Icelandic glacier Vatnajokull.</obo:IAO_0000115>
        <oboInOwl:hasOBONamespace>GAZ</oboInOwl:hasOBONamespace>
        <oboInOwl:id>GAZ:00062058</oboInOwl:id>
        <rdfs:label>Fjallsarlon</rdfs:label>
    </owl:NamedIndividual>
    


    <!-- http://purl.obolibrary.org/obo/GAZ_00062059 -->

    <owl:NamedIndividual rdf:about="http://purl.obolibrary.org/obo/GAZ_00062059">
        <obo:RO_0001025 rdf:resource="http://purl.obolibrary.org/obo/GAZ_00001204"/>
        <obo:IAO_0000115>A lake in Iceland. It is situated in the Highlands of Iceland, not far from the famous mountains of Landmannalaugar and the volcano Hekla.</obo:IAO_0000115>
        <oboInOwl:hasOBONamespace>GAZ</oboInOwl:hasOBONamespace>
        <oboInOwl:id>GAZ:00062059</oboInOwl:id>
        <rdfs:label>Frostastadavatn</rdfs:label>
    </owl:NamedIndividual>
    


    <!-- http://purl.obolibrary.org/obo/GAZ_00062060 -->

    <owl:NamedIndividual rdf:about="http://purl.obolibrary.org/obo/GAZ_00062060">
        <obo:RO_0001025 rdf:resource="http://purl.obolibrary.org/obo/GAZ_00001204"/>
        <obo:RO_0001025 rdf:resource="http://purl.obolibrary.org/obo/GAZ_00053316"/>
        <obo:IAO_0000115>Glacier lakes of the Icelandic glacier Vatnajokull. Itis situated in the south of Iceland.</obo:IAO_0000115>
        <oboInOwl:hasOBONamespace>GAZ</oboInOwl:hasOBONamespace>
        <oboInOwl:id>GAZ:00062060</oboInOwl:id>
        <rdfs:label>Graenalon</rdfs:label>
    </owl:NamedIndividual>
    


    <!-- http://purl.obolibrary.org/obo/GAZ_00062061 -->

    <owl:NamedIndividual rdf:about="http://purl.obolibrary.org/obo/GAZ_00062061">
        <obo:RO_0001025 rdf:resource="http://purl.obolibrary.org/obo/GAZ_00053316"/>
        <obo:IAO_0000115>Subglacial lakes in Iceland. They lie in the highlands of Iceland at the northwestern side of the Vatnajokull glacier and are covered by its ice cap. Beneath them is a large magma chamber of a powerful volcano.</obo:IAO_0000115>
        <oboInOwl:hasOBONamespace>GAZ</oboInOwl:hasOBONamespace>
        <oboInOwl:id>GAZ:00062061</oboInOwl:id>
        <rdfs:label>Grimsvotn [lakes]</rdfs:label>
    </owl:NamedIndividual>
    


    <!-- http://purl.obolibrary.org/obo/GAZ_00062062 -->

    <owl:NamedIndividual rdf:about="http://purl.obolibrary.org/obo/GAZ_00062062">
        <obo:RO_0001025 rdf:resource="http://purl.obolibrary.org/obo/GAZ_00001206"/>
        <obo:IAO_0000115>A lake in the west of Iceland. It is situated near Route 1 (the Ring Road) between Borgarnes and the pass of Holtavortuheidi.</obo:IAO_0000115>
        <oboInOwl:hasOBONamespace>GAZ</oboInOwl:hasOBONamespace>
        <oboInOwl:id>GAZ:00062062</oboInOwl:id>
        <rdfs:label>Hredavatn</rdfs:label>
    </owl:NamedIndividual>
    


    <!-- http://purl.obolibrary.org/obo/GAZ_00062063 -->

    <owl:NamedIndividual rdf:about="http://purl.obolibrary.org/obo/GAZ_00062063">
        <obo:RO_0001025 rdf:resource="http://purl.obolibrary.org/obo/GAZ_00001206"/>
        <obo:IAO_0000115>An extinct volcano situated in the west of Iceland next to Route 1.</obo:IAO_0000115>
        <oboInOwl:hasOBONamespace>GAZ</oboInOwl:hasOBONamespace>
        <oboInOwl:id>GAZ:00062063</oboInOwl:id>
        <rdfs:label>Baula</rdfs:label>
    </owl:NamedIndividual>
    


    <!-- http://purl.obolibrary.org/obo/GAZ_00062064 -->

    <owl:NamedIndividual rdf:about="http://purl.obolibrary.org/obo/GAZ_00062064">
        <obo:RO_0001025 rdf:resource="http://purl.obolibrary.org/obo/GAZ_00001206"/>
        <obo:IAO_0000115>A lake located some km to the east of Hvalfjoerdur in the western portion of Iceland. It lies to the east of the volcano Hvalfell.</obo:IAO_0000115>
        <oboInOwl:hasOBONamespace>GAZ</oboInOwl:hasOBONamespace>
        <oboInOwl:id>GAZ:00062064</oboInOwl:id>
        <rdfs:label>Hvalvatn</rdfs:label>
    </owl:NamedIndividual>
    


    <!-- http://purl.obolibrary.org/obo/GAZ_00062065 -->

    <owl:NamedIndividual rdf:about="http://purl.obolibrary.org/obo/GAZ_00062065">
        <obo:RO_0001025 rdf:resource="http://purl.obolibrary.org/obo/GAZ_00001204"/>
        <obo:IAO_0000115>A small lake in the southern Highlands of Iceland. It is situated between Sidujokull and Skeitharajokull, two of the southern arms of the big glacier Vatnajokull, and lies 15 km to the north of the infamous Skeithara sander.</obo:IAO_0000115>
        <oboInOwl:hasOBONamespace>GAZ</oboInOwl:hasOBONamespace>
        <oboInOwl:id>GAZ:00062065</oboInOwl:id>
        <rdfs:label>Hvitavatn</rdfs:label>
    </owl:NamedIndividual>
    


    <!-- http://purl.obolibrary.org/obo/GAZ_00062066 -->

    <owl:NamedIndividual rdf:about="http://purl.obolibrary.org/obo/GAZ_00062066">
        <obo:RO_0001025 rdf:resource="http://purl.obolibrary.org/obo/GAZ_00001204"/>
        <obo:IAO_0000115>A lake in the Highlands of Iceland and the source of glacial river Hvita. It is located 45 km northeast of Gullfoss.</obo:IAO_0000115>
        <oboInOwl:hasOBONamespace>GAZ</oboInOwl:hasOBONamespace>
        <oboInOwl:id>GAZ:00062066</oboInOwl:id>
        <rdfs:label>Hvitarvatn</rdfs:label>
    </owl:NamedIndividual>
    


    <!-- http://purl.obolibrary.org/obo/GAZ_00062068 -->

    <owl:NamedIndividual rdf:about="http://purl.obolibrary.org/obo/GAZ_00062068">
        <obo:RO_0001025 rdf:resource="http://purl.obolibrary.org/obo/GAZ_00001203"/>
        <obo:RO_0001025 rdf:resource="http://purl.obolibrary.org/obo/GAZ_00053316"/>
        <obo:IAO_0000115>A glacial lake in Iceland. It is situated at the south end of the glacier Vatnajokull between Skaftafell National Park and Hofn. Appearing first only in 1934-1935, the lake grew from 7.9 km2 in 1975 to at least 18 km2 today because of heavy melting of the Icelandic glaciers.</obo:IAO_0000115>
        <oboInOwl:hasOBONamespace>GAZ</oboInOwl:hasOBONamespace>
        <oboInOwl:id>GAZ:00062068</oboInOwl:id>
        <rdfs:label>Jokulsarlon</rdfs:label>
    </owl:NamedIndividual>
    


    <!-- http://purl.obolibrary.org/obo/GAZ_00062069 -->

    <owl:NamedIndividual rdf:about="http://purl.obolibrary.org/obo/GAZ_00062069">
        <obo:RO_0001025 rdf:resource="http://purl.obolibrary.org/obo/GAZ_00008736"/>
        <obo:IAO_0000115>A lake on the Reykjanes peninsula in Iceland.</obo:IAO_0000115>
        <oboInOwl:hasOBONamespace>GAZ</oboInOwl:hasOBONamespace>
        <oboInOwl:id>GAZ:00062069</oboInOwl:id>
        <rdfs:label>Kleifarvatn</rdfs:label>
    </owl:NamedIndividual>
    


    <!-- http://purl.obolibrary.org/obo/GAZ_00062070 -->

    <owl:NamedIndividual rdf:about="http://purl.obolibrary.org/obo/GAZ_00062070">
        <obo:RO_0001025 rdf:resource="http://purl.obolibrary.org/obo/GAZ_00001204"/>
        <obo:IAO_0000115>A lake located in the Highlands of Iceland to the west of Sprengisandur highland road and to the south-east of the glacier Hofsjokull.</obo:IAO_0000115>
        <oboInOwl:hasOBONamespace>GAZ</oboInOwl:hasOBONamespace>
        <oboInOwl:id>GAZ:00062070</oboInOwl:id>
        <rdfs:label>Kvislavatn</rdfs:label>
    </owl:NamedIndividual>
    


    <!-- http://purl.obolibrary.org/obo/GAZ_00062071 -->

    <owl:NamedIndividual rdf:about="http://purl.obolibrary.org/obo/GAZ_00062071">
        <obo:RO_0001025 rdf:resource="http://purl.obolibrary.org/obo/GAZ_00020005"/>
        <obo:IAO_0000115>A lake located in the east of Iceland near Egilsstadir.</obo:IAO_0000115>
        <oboInOwl:hasOBONamespace>GAZ</oboInOwl:hasOBONamespace>
        <oboInOwl:id>GAZ:00062071</oboInOwl:id>
        <rdfs:label>Lagarfljot</rdfs:label>
    </owl:NamedIndividual>
    


    <!-- http://purl.obolibrary.org/obo/GAZ_00062072 -->

    <owl:NamedIndividual rdf:about="http://purl.obolibrary.org/obo/GAZ_00062072">
        <obo:RO_0001025 rdf:resource="http://purl.obolibrary.org/obo/GAZ_00001204"/>
        <obo:IAO_0000115>A reservoir in Iceland, located in the south of the country, not far from Landmannalaugar.</obo:IAO_0000115>
        <oboInOwl:hasOBONamespace>GAZ</oboInOwl:hasOBONamespace>
        <oboInOwl:id>GAZ:00062072</oboInOwl:id>
        <rdfs:label>Sigoldulon</rdfs:label>
    </owl:NamedIndividual>
    


    <!-- http://purl.obolibrary.org/obo/GAZ_00062073 -->

    <owl:NamedIndividual rdf:about="http://purl.obolibrary.org/obo/GAZ_00062073">
        <obo:RO_0001025 rdf:resource="http://purl.obolibrary.org/obo/GAZ_00001204"/>
        <obo:IAO_0000115>A reservoir the Highlands of Iceland to the north of the volcano Hekla. It is a reservoir of the river Thjorsa. Its surface is measuring 19 km2.</obo:IAO_0000115>
        <oboInOwl:hasOBONamespace>GAZ</oboInOwl:hasOBONamespace>
        <oboInOwl:id>GAZ:00062073</oboInOwl:id>
        <rdfs:label>Sultartangalon</rdfs:label>
    </owl:NamedIndividual>
    


    <!-- http://purl.obolibrary.org/obo/GAZ_00062074 -->

    <owl:NamedIndividual rdf:about="http://purl.obolibrary.org/obo/GAZ_00062074">
        <obo:RO_0001025 rdf:resource="http://purl.obolibrary.org/obo/GAZ_00001204"/>
        <obo:IAO_0000115>A lake in the Highlands of Iceland. It is located at the south-western border of Vatnajokull at an altitude of 670 m above sea level.</obo:IAO_0000115>
        <oboInOwl:hasOBONamespace>GAZ</oboInOwl:hasOBONamespace>
        <oboInOwl:id>GAZ:00062074</oboInOwl:id>
        <rdfs:label>Langisjor</rdfs:label>
    </owl:NamedIndividual>
    


    <!-- http://purl.obolibrary.org/obo/GAZ_00062075 -->

    <owl:NamedIndividual rdf:about="http://purl.obolibrary.org/obo/GAZ_00062075">
        <obo:RO_0001025 rdf:resource="http://purl.obolibrary.org/obo/GAZ_00020020"/>
        <obo:IAO_0000115>A shallow eutrophic lake situated in an area of active volcanism in the north of Iceland, not far from Krafla volcano. The lake was created by a large basaltic lava eruption 2300 years ago, and the surrounding landscape is dominated by volcanic landforms, including lava pillars and rootless vents (pseudocraters).</obo:IAO_0000115>
        <oboInOwl:hasOBONamespace>GAZ</oboInOwl:hasOBONamespace>
        <oboInOwl:id>GAZ:00062075</oboInOwl:id>
        <rdfs:label>Myvatn</rdfs:label>
    </owl:NamedIndividual>
    


    <!-- http://purl.obolibrary.org/obo/GAZ_00062076 -->

    <owl:NamedIndividual rdf:about="http://purl.obolibrary.org/obo/GAZ_00062076">
        <obo:RO_0001025 rdf:resource="http://purl.obolibrary.org/obo/GAZ_00001206"/>
        <obo:IAO_0000115>A lake in the west of Iceland. It is situated in a narrow valley between the Hvalfjoerdur and the valley Reykholtsdalur. The lake is also a reservoir so that the level of the water surface has been raised artificially.</obo:IAO_0000115>
        <oboInOwl:hasOBONamespace>GAZ</oboInOwl:hasOBONamespace>
        <oboInOwl:id>GAZ:00062076</oboInOwl:id>
        <rdfs:label>Skorradalsvatn</rdfs:label>
    </owl:NamedIndividual>
    


    <!-- http://purl.obolibrary.org/obo/GAZ_00062077 -->

    <owl:NamedIndividual rdf:about="http://purl.obolibrary.org/obo/GAZ_00062077">
        <obo:RO_0001025 rdf:resource="http://purl.obolibrary.org/obo/GAZ_00001204"/>
        <obo:IAO_0000115>A lake in the south of Iceland.</obo:IAO_0000115>
        <oboInOwl:hasOBONamespace>GAZ</oboInOwl:hasOBONamespace>
        <oboInOwl:id>GAZ:00062077</oboInOwl:id>
        <rdfs:label>Laugarvatn</rdfs:label>
    </owl:NamedIndividual>
    


    <!-- http://purl.obolibrary.org/obo/GAZ_00062078 -->

    <owl:NamedIndividual rdf:about="http://purl.obolibrary.org/obo/GAZ_00062078">
        <obo:RO_0001025 rdf:resource="http://purl.obolibrary.org/obo/GAZ_00053318"/>
        <obo:IAO_0000115>A crater lake in the Highlands of Iceland.</obo:IAO_0000115>
        <oboInOwl:hasOBONamespace>GAZ</oboInOwl:hasOBONamespace>
        <oboInOwl:id>GAZ:00062078</oboInOwl:id>
        <rdfs:label>Oskjuvatn</rdfs:label>
    </owl:NamedIndividual>
    


    <!-- http://purl.obolibrary.org/obo/GAZ_00062079 -->

    <owl:NamedIndividual rdf:about="http://purl.obolibrary.org/obo/GAZ_00062079">
        <obo:RO_0001025 rdf:resource="http://purl.obolibrary.org/obo/GAZ_00280119"/>
        <obo:IAO_0000115>The largest body of water on Ofeigsfjardarheitdi in Iceland.</obo:IAO_0000115>
        <oboInOwl:hasOBONamespace>GAZ</oboInOwl:hasOBONamespace>
        <oboInOwl:id>GAZ:00062079</oboInOwl:id>
        <rdfs:label>Nyrdra-Vatnalautavatn</rdfs:label>
    </owl:NamedIndividual>
    


    <!-- http://purl.obolibrary.org/obo/GAZ_00062080 -->

    <owl:NamedIndividual rdf:about="http://purl.obolibrary.org/obo/GAZ_00062080">
        <obo:RO_0001025 rdf:resource="http://purl.obolibrary.org/obo/GAZ_00001202"/>
        <obo:IAO_0000115>A lake to the south of Blonduos.</obo:IAO_0000115>
        <oboInOwl:hasOBONamespace>GAZ</oboInOwl:hasOBONamespace>
        <oboInOwl:id>GAZ:00062080</oboInOwl:id>
        <rdfs:label>Svinavatn [Blonduos]</rdfs:label>
    </owl:NamedIndividual>
    


    <!-- http://purl.obolibrary.org/obo/GAZ_00062081 -->

    <owl:NamedIndividual rdf:about="http://purl.obolibrary.org/obo/GAZ_00062081">
        <obo:RO_0001025 rdf:resource="http://purl.obolibrary.org/obo/GAZ_00280116"/>
        <obo:IAO_0000115>A reservoir located at the south end of Sprengisandur highland road within the highlands of Iceland.</obo:IAO_0000115>
        <oboInOwl:hasOBONamespace>GAZ</oboInOwl:hasOBONamespace>
        <oboInOwl:id>GAZ:00062081</oboInOwl:id>
        <rdfs:label>Thorisvatn</rdfs:label>
    </owl:NamedIndividual>
    


    <!-- http://purl.obolibrary.org/obo/GAZ_00062082 -->

    <owl:NamedIndividual rdf:about="http://purl.obolibrary.org/obo/GAZ_00062082">
        <obo:RO_0001025 rdf:resource="http://purl.obolibrary.org/obo/GAZ_00001202"/>
        <obo:IAO_0000115>A lake in Iceland.</obo:IAO_0000115>
        <oboInOwl:hasOBONamespace>GAZ</oboInOwl:hasOBONamespace>
        <oboInOwl:id>GAZ:00062082</oboInOwl:id>
        <rdfs:label>Hofdavatn</rdfs:label>
    </owl:NamedIndividual>
    


    <!-- http://purl.obolibrary.org/obo/GAZ_00062083 -->

    <owl:NamedIndividual rdf:about="http://purl.obolibrary.org/obo/GAZ_00062083">
        <obo:RO_0001025 rdf:resource="http://purl.obolibrary.org/obo/GAZ_00008737"/>
        <obo:IAO_0000115>A small lake in central Reykjavik, the capital of Iceland.</obo:IAO_0000115>
        <oboInOwl:hasOBONamespace>GAZ</oboInOwl:hasOBONamespace>
        <oboInOwl:id>GAZ:00062083</oboInOwl:id>
        <rdfs:label>Tjornin</rdfs:label>
    </owl:NamedIndividual>
    


    <!-- http://purl.obolibrary.org/obo/GAZ_00062084 -->

    <owl:NamedIndividual rdf:about="http://purl.obolibrary.org/obo/GAZ_00062084">
        <obo:RO_0001025 rdf:resource="http://purl.obolibrary.org/obo/GAZ_00062086"/>
        <obo:IAO_0000115>A very small lake in the valley Heydalur near Hvammsfjoerdur on the peninsula of Snaefellsnes.</obo:IAO_0000115>
        <oboInOwl:hasOBONamespace>GAZ</oboInOwl:hasOBONamespace>
        <oboInOwl:id>GAZ:00062084</oboInOwl:id>
        <rdfs:label>Svinavatn [Heydalur]</rdfs:label>
    </owl:NamedIndividual>
    


    <!-- http://purl.obolibrary.org/obo/GAZ_00062085 -->

    <owl:NamedIndividual rdf:about="http://purl.obolibrary.org/obo/GAZ_00062085">
        <obo:RO_0001025 rdf:resource="http://purl.obolibrary.org/obo/GAZ_00001202"/>
        <obo:IAO_0000115>A lake to the west of Blondulon at the north end of Kjolur highland road.</obo:IAO_0000115>
        <oboInOwl:hasOBONamespace>GAZ</oboInOwl:hasOBONamespace>
        <oboInOwl:id>GAZ:00062085</oboInOwl:id>
        <rdfs:label>Svinavatn [Blondulon]</rdfs:label>
    </owl:NamedIndividual>
    


    <!-- http://purl.obolibrary.org/obo/GAZ_00062086 -->

    <owl:NamedIndividual rdf:about="http://purl.obolibrary.org/obo/GAZ_00062086">
        <obo:RO_0001025 rdf:resource="http://purl.obolibrary.org/obo/GAZ_00001206"/>
        <obo:IAO_0000115>A peninsula situated to the west of Borgarfjoerdur in the west of Iceland.</obo:IAO_0000115>
        <oboInOwl:hasOBONamespace>GAZ</oboInOwl:hasOBONamespace>
        <oboInOwl:id>GAZ:00062086</oboInOwl:id>
        <rdfs:label>Snaefellsnes Peninsula</rdfs:label>
    </owl:NamedIndividual>
    


    <!-- http://purl.obolibrary.org/obo/GAZ_00062087 -->

    <owl:NamedIndividual rdf:about="http://purl.obolibrary.org/obo/GAZ_00062087">
        <obo:RO_0001025 rdf:resource="http://purl.obolibrary.org/obo/GAZ_00001204"/>
        <obo:IAO_0000115>A lake in Iceland.</obo:IAO_0000115>
        <oboInOwl:hasOBONamespace>GAZ</oboInOwl:hasOBONamespace>
        <oboInOwl:id>GAZ:00062087</oboInOwl:id>
        <rdfs:label>Hestvatn</rdfs:label>
    </owl:NamedIndividual>
    


    <!-- http://purl.obolibrary.org/obo/GAZ_00062088 -->

    <owl:NamedIndividual rdf:about="http://purl.obolibrary.org/obo/GAZ_00062088">
        <obo:RO_0001025 rdf:resource="http://purl.obolibrary.org/obo/GAZ_00001202"/>
        <obo:IAO_0000115>A lake in Iceland.</obo:IAO_0000115>
        <oboInOwl:hasOBONamespace>GAZ</oboInOwl:hasOBONamespace>
        <oboInOwl:id>GAZ:00062088</oboInOwl:id>
        <rdfs:label>Vesturhopsvatn</rdfs:label>
    </owl:NamedIndividual>
    


    <!-- http://purl.obolibrary.org/obo/GAZ_00089838 -->

    <owl:NamedIndividual rdf:about="http://purl.obolibrary.org/obo/GAZ_00089838">
        <obo:RO_0001025 rdf:resource="http://purl.obolibrary.org/obo/GAZ_00001207"/>
        <obo:IAO_0000115>A national park situated in the north of Iceland around the river Jokulsa a Fjollum. It lies to the north of the Dettifoss waterfall.</obo:IAO_0000115>
        <oboInOwl:hasOBONamespace>GAZ</oboInOwl:hasOBONamespace>
        <oboInOwl:id>GAZ:00089838</oboInOwl:id>
        <rdfs:label>Jokulsargljufur National Park</rdfs:label>
    </owl:NamedIndividual>
    


    <!-- http://purl.obolibrary.org/obo/GAZ_00089839 -->

    <owl:NamedIndividual rdf:about="http://purl.obolibrary.org/obo/GAZ_00089839">
        <obo:RO_0001025 rdf:resource="http://purl.obolibrary.org/obo/GAZ_00062086"/>
        <obo:IAO_0000115>A protected area.</obo:IAO_0000115>
        <oboInOwl:hasOBONamespace>GAZ</oboInOwl:hasOBONamespace>
        <oboInOwl:id>GAZ:00089839</oboInOwl:id>
        <rdfs:label>Snaefellsjokull National Park</rdfs:label>
    </owl:NamedIndividual>
    


    <!-- http://purl.obolibrary.org/obo/GAZ_00145753 -->

    <owl:NamedIndividual rdf:about="http://purl.obolibrary.org/obo/GAZ_00145753">
        <obo:RO_0001025 rdf:resource="http://purl.obolibrary.org/obo/GAZ_00000843"/>
        <oboInOwl:hasOBONamespace>GAZ</oboInOwl:hasOBONamespace>
        <oboInOwl:id>GAZ:00145753</oboInOwl:id>
        <rdfs:label>Coastal waters of Iceland</rdfs:label>
    </owl:NamedIndividual>
    


    <!-- http://purl.obolibrary.org/obo/GAZ_00145754 -->

    <owl:NamedIndividual rdf:about="http://purl.obolibrary.org/obo/GAZ_00145754">
        <obo:RO_0001025 rdf:resource="http://purl.obolibrary.org/obo/GAZ_00280523"/>
        <obo:IAO_0000115>A bay in southwest Iceland between the peninsulas of Snaefellsnes and Reykjanes. The capital of the island, Reykjavik, is situated on its southern shore.</obo:IAO_0000115>
        <oboInOwl:hasOBONamespace>GAZ</oboInOwl:hasOBONamespace>
        <oboInOwl:id>GAZ:00145754</oboInOwl:id>
        <rdfs:label>Faxafloi</rdfs:label>
    </owl:NamedIndividual>
    


    <!-- http://purl.obolibrary.org/obo/GAZ_00145755 -->

    <owl:NamedIndividual rdf:about="http://purl.obolibrary.org/obo/GAZ_00145755">
        <obo:RO_0001025 rdf:resource="http://purl.obolibrary.org/obo/GAZ_00020056"/>
        <obo:RO_0001025 rdf:resource="http://purl.obolibrary.org/obo/GAZ_00280523"/>
        <obo:IAO_0000115>A large fjord in the Westfjords region of Iceland.</obo:IAO_0000115>
        <oboInOwl:hasOBONamespace>GAZ</oboInOwl:hasOBONamespace>
        <oboInOwl:id>GAZ:00145755</oboInOwl:id>
        <rdfs:label>Isafjardardjup</rdfs:label>
    </owl:NamedIndividual>
    


    <!-- http://purl.obolibrary.org/obo/GAZ_00145756 -->

    <owl:NamedIndividual rdf:about="http://purl.obolibrary.org/obo/GAZ_00145756">
        <obo:RO_0001025 rdf:resource="http://purl.obolibrary.org/obo/GAZ_00001206"/>
        <obo:RO_0001025 rdf:resource="http://purl.obolibrary.org/obo/GAZ_00145754"/>
        <obo:IAO_0000115>A fjord in the west of Iceland near the town of Borgarnes.</obo:IAO_0000115>
        <oboInOwl:hasOBONamespace>GAZ</oboInOwl:hasOBONamespace>
        <oboInOwl:id>GAZ:00145756</oboInOwl:id>
        <rdfs:label>Borgarfjoerdur [W]</rdfs:label>
    </owl:NamedIndividual>
    


    <!-- http://purl.obolibrary.org/obo/GAZ_00145757 -->

    <owl:NamedIndividual rdf:about="http://purl.obolibrary.org/obo/GAZ_00145757">
        <obo:RO_0001025 rdf:resource="http://purl.obolibrary.org/obo/GAZ_00053332"/>
        <obo:IAO_0000115>An island in the Skagafjoerdur.</obo:IAO_0000115>
        <oboInOwl:hasOBONamespace>GAZ</oboInOwl:hasOBONamespace>
        <oboInOwl:id>GAZ:00145757</oboInOwl:id>
        <rdfs:label>Lundey</rdfs:label>
    </owl:NamedIndividual>
    


    <!-- http://purl.obolibrary.org/obo/GAZ_00145758 -->

    <owl:NamedIndividual rdf:about="http://purl.obolibrary.org/obo/GAZ_00145758">
        <obo:RO_0001025 rdf:resource="http://purl.obolibrary.org/obo/GAZ_00001202"/>
        <obo:RO_0001025 rdf:resource="http://purl.obolibrary.org/obo/GAZ_00280522"/>
        <obo:IAO_0000115>A large bay between Strandir and Skagastrond in Iceland. It is about 50 km wide and 100 km long. The towns Blonduos and Skagastrond are located on the bay&apos;s eastern side.</obo:IAO_0000115>
        <oboInOwl:hasOBONamespace>GAZ</oboInOwl:hasOBONamespace>
        <oboInOwl:id>GAZ:00145758</oboInOwl:id>
        <rdfs:label>Hunafloi</rdfs:label>
    </owl:NamedIndividual>
    


    <!-- http://purl.obolibrary.org/obo/GAZ_00145759 -->

    <owl:NamedIndividual rdf:about="http://purl.obolibrary.org/obo/GAZ_00145759">
        <obo:RO_0001025 rdf:resource="http://purl.obolibrary.org/obo/GAZ_00001206"/>
        <obo:RO_0001025 rdf:resource="http://purl.obolibrary.org/obo/GAZ_00145754"/>
        <obo:IAO_0000115>A fjord situated in the west of Iceland between Mosfellsbaer and Akranes. The fjord is approximately 30 km long and 5 km wide.</obo:IAO_0000115>
        <oboInOwl:hasOBONamespace>GAZ</oboInOwl:hasOBONamespace>
        <oboInOwl:id>GAZ:00145759</oboInOwl:id>
        <rdfs:label>Hvalfjoerdur</rdfs:label>
    </owl:NamedIndividual>
    


    <!-- http://purl.obolibrary.org/obo/GAZ_00145760 -->

    <owl:NamedIndividual rdf:about="http://purl.obolibrary.org/obo/GAZ_00145760">
        <obo:RO_0001025 rdf:resource="http://purl.obolibrary.org/obo/GAZ_00001204"/>
        <obo:RO_0001025 rdf:resource="http://purl.obolibrary.org/obo/GAZ_00280523"/>
        <obo:IAO_0000115>Basalt sea stacks situated under the mountain Reynisfjall near the village Vik i Myrdal, southern Iceland.</obo:IAO_0000115>
        <oboInOwl:hasOBONamespace>GAZ</oboInOwl:hasOBONamespace>
        <oboInOwl:id>GAZ:00145760</oboInOwl:id>
        <rdfs:label>Reynisdrangar</rdfs:label>
    </owl:NamedIndividual>
    


    <!-- http://purl.obolibrary.org/obo/GAZ_00145761 -->

    <owl:NamedIndividual rdf:about="http://purl.obolibrary.org/obo/GAZ_00145761">
        <obo:RO_0001025 rdf:resource="http://purl.obolibrary.org/obo/GAZ_00001207"/>
        <obo:RO_0001025 rdf:resource="http://purl.obolibrary.org/obo/GAZ_00280522"/>
        <obo:IAO_0000115>A broad fjord in northeastern Iceland, situated between the Tjornes and Melrakkasletta headlands.</obo:IAO_0000115>
        <oboInOwl:hasOBONamespace>GAZ</oboInOwl:hasOBONamespace>
        <oboInOwl:id>GAZ:00145761</oboInOwl:id>
        <rdfs:label>Oxarfjoerdur</rdfs:label>
    </owl:NamedIndividual>
    


    <!-- http://purl.obolibrary.org/obo/GAZ_00145763 -->

    <owl:NamedIndividual rdf:about="http://purl.obolibrary.org/obo/GAZ_00145763">
        <obo:RO_0001025 rdf:resource="http://purl.obolibrary.org/obo/GAZ_00053333"/>
        <obo:IAO_0000115>The narrowest part of the Breidhafjrdhur.</obo:IAO_0000115>
        <oboInOwl:hasOBONamespace>GAZ</oboInOwl:hasOBONamespace>
        <oboInOwl:id>GAZ:00145763</oboInOwl:id>
        <rdfs:label>Hvammsfjoerdur</rdfs:label>
    </owl:NamedIndividual>
    


    <!-- http://purl.obolibrary.org/obo/GAZ_00145764 -->

    <owl:NamedIndividual rdf:about="http://purl.obolibrary.org/obo/GAZ_00145764">
        <obo:RO_0001025 rdf:resource="http://purl.obolibrary.org/obo/GAZ_00001205"/>
        <obo:IAO_0000115>A peninsula in northwestern Iceland. It is connected to the rest of Iceland by a 7 km wide isthmus between Gilsfjoerdur and Bitrufjoerdur.</obo:IAO_0000115>
        <oboInOwl:hasOBONamespace>GAZ</oboInOwl:hasOBONamespace>
        <oboInOwl:id>GAZ:00145764</oboInOwl:id>
        <rdfs:label>Westfjords Peninsula</rdfs:label>
    </owl:NamedIndividual>
    


    <!-- http://purl.obolibrary.org/obo/GAZ_00145765 -->

    <owl:NamedIndividual rdf:about="http://purl.obolibrary.org/obo/GAZ_00145765">
        <obo:RO_0001025 rdf:resource="http://purl.obolibrary.org/obo/GAZ_00145764"/>
        <obo:IAO_0000115>A peninsula in the Westfjords. Located to the north of the Jokulfirdir and to the northwest of Drangajdkull.</obo:IAO_0000115>
        <oboInOwl:hasOBONamespace>GAZ</oboInOwl:hasOBONamespace>
        <oboInOwl:id>GAZ:00145765</oboInOwl:id>
        <rdfs:label>Hornstrandir</rdfs:label>
    </owl:NamedIndividual>
    


    <!-- http://purl.obolibrary.org/obo/GAZ_00145766 -->

    <owl:NamedIndividual rdf:about="http://purl.obolibrary.org/obo/GAZ_00145766">
        <obo:RO_0001025 rdf:resource="http://purl.obolibrary.org/obo/GAZ_00001204"/>
        <obo:IAO_0000115>A peninsula located on the south coast of Iceland, not far from Vik i Myrdal. It is a former island of volcanic origin.</obo:IAO_0000115>
        <oboInOwl:hasOBONamespace>GAZ</oboInOwl:hasOBONamespace>
        <oboInOwl:id>GAZ:00145766</oboInOwl:id>
        <rdfs:label>Dyrholaey</rdfs:label>
    </owl:NamedIndividual>
    


    <!-- http://purl.obolibrary.org/obo/GAZ_00145767 -->

    <owl:NamedIndividual rdf:about="http://purl.obolibrary.org/obo/GAZ_00145767">
        <obo:RO_0001025 rdf:resource="http://purl.obolibrary.org/obo/GAZ_00001207"/>
        <obo:IAO_0000115>A peninsula in northeast Iceland, located to the west of the Fontur peninsula.</obo:IAO_0000115>
        <oboInOwl:hasOBONamespace>GAZ</oboInOwl:hasOBONamespace>
        <oboInOwl:id>GAZ:00145767</oboInOwl:id>
        <rdfs:label>Rifstangi</rdfs:label>
    </owl:NamedIndividual>
    


    <!-- http://purl.obolibrary.org/obo/GAZ_00145768 -->

    <owl:NamedIndividual rdf:about="http://purl.obolibrary.org/obo/GAZ_00145768">
        <obo:RO_0001025 rdf:resource="http://purl.obolibrary.org/obo/GAZ_00001207"/>
        <obo:IAO_0000115>A large peninsula on the northeastern tip of Iceland. It is located in-between the Thistilfjoerdur and Bakkafloi fjords.</obo:IAO_0000115>
        <oboInOwl:hasOBONamespace>GAZ</oboInOwl:hasOBONamespace>
        <oboInOwl:id>GAZ:00145768</oboInOwl:id>
        <rdfs:label>Fontur</rdfs:label>
    </owl:NamedIndividual>
    


    <!-- http://purl.obolibrary.org/obo/GAZ_00145770 -->

    <owl:NamedIndividual rdf:about="http://purl.obolibrary.org/obo/GAZ_00145770">
        <obo:RO_0001025 rdf:resource="http://purl.obolibrary.org/obo/GAZ_00001204"/>
        <obo:IAO_0000115>A sandur. A broad sandy wasteland along Iceland&apos;s south-eastern coast, between the Vatnajokull icecap and the sea.</obo:IAO_0000115>
        <oboInOwl:hasOBONamespace>GAZ</oboInOwl:hasOBONamespace>
        <oboInOwl:id>GAZ:00145770</oboInOwl:id>
        <rdfs:label>Skeidararsandur</rdfs:label>
    </owl:NamedIndividual>
    


    <!-- http://purl.obolibrary.org/obo/GAZ_00145771 -->

    <owl:NamedIndividual rdf:about="http://purl.obolibrary.org/obo/GAZ_00145771">
        <obo:RO_0001025 rdf:resource="http://purl.obolibrary.org/obo/GAZ_00020009"/>
        <obo:RO_0001025 rdf:resource="http://purl.obolibrary.org/obo/GAZ_00053321"/>
        <obo:IAO_0000115>A fjord in NE Iceland.</obo:IAO_0000115>
        <oboInOwl:hasOBONamespace>GAZ</oboInOwl:hasOBONamespace>
        <oboInOwl:id>GAZ:00145771</oboInOwl:id>
        <rdfs:label>Vopnafjoerdur</rdfs:label>
    </owl:NamedIndividual>
    


    <!-- http://purl.obolibrary.org/obo/GAZ_00145772 -->

    <owl:NamedIndividual rdf:about="http://purl.obolibrary.org/obo/GAZ_00145772">
        <obo:RO_0001025 rdf:resource="http://purl.obolibrary.org/obo/GAZ_00001203"/>
        <obo:RO_0001025 rdf:resource="http://purl.obolibrary.org/obo/GAZ_00280522"/>
        <obo:IAO_0000115>A fjord in E Iceland.</obo:IAO_0000115>
        <oboInOwl:hasOBONamespace>GAZ</oboInOwl:hasOBONamespace>
        <oboInOwl:id>GAZ:00145772</oboInOwl:id>
        <rdfs:label>Seydisfjoerdur [East]</rdfs:label>
    </owl:NamedIndividual>
    


    <!-- http://purl.obolibrary.org/obo/GAZ_00145773 -->

    <owl:NamedIndividual rdf:about="http://purl.obolibrary.org/obo/GAZ_00145773">
        <obo:RO_0001025 rdf:resource="http://purl.obolibrary.org/obo/GAZ_00020004"/>
        <obo:RO_0001025 rdf:resource="http://purl.obolibrary.org/obo/GAZ_00280523"/>
        <obo:IAO_0000115>A fjord in E Iceland.</obo:IAO_0000115>
        <oboInOwl:hasOBONamespace>GAZ</oboInOwl:hasOBONamespace>
        <oboInOwl:id>GAZ:00145773</oboInOwl:id>
        <rdfs:label>Reydarfjoerdur</rdfs:label>
    </owl:NamedIndividual>
    


    <!-- http://purl.obolibrary.org/obo/GAZ_00145774 -->

    <owl:NamedIndividual rdf:about="http://purl.obolibrary.org/obo/GAZ_00145774">
        <obo:RO_0001025 rdf:resource="http://purl.obolibrary.org/obo/GAZ_00280516"/>
        <obo:IAO_0000115>A fjord in E Iceland.</obo:IAO_0000115>
        <oboInOwl:hasOBONamespace>GAZ</oboInOwl:hasOBONamespace>
        <oboInOwl:id>GAZ:00145774</oboInOwl:id>
        <rdfs:label>Nordfjoerdur</rdfs:label>
    </owl:NamedIndividual>
    


    <!-- http://purl.obolibrary.org/obo/GAZ_00145775 -->

    <owl:NamedIndividual rdf:about="http://purl.obolibrary.org/obo/GAZ_00145775">
        <obo:RO_0001025 rdf:resource="http://purl.obolibrary.org/obo/GAZ_00145764"/>
        <obo:RO_0001025 rdf:resource="http://purl.obolibrary.org/obo/GAZ_00280522"/>
        <obo:IAO_0000115>A fjord in the north-west of Iceland. It is around 36 km long and lies to the south of Hunafloi bay.</obo:IAO_0000115>
        <oboInOwl:hasOBONamespace>GAZ</oboInOwl:hasOBONamespace>
        <oboInOwl:id>GAZ:00145775</oboInOwl:id>
        <rdfs:label>Hrutafjoerdur</rdfs:label>
    </owl:NamedIndividual>
    


    <!-- http://purl.obolibrary.org/obo/GAZ_00145776 -->

    <owl:NamedIndividual rdf:about="http://purl.obolibrary.org/obo/GAZ_00145776">
        <obo:RO_0001025 rdf:resource="http://purl.obolibrary.org/obo/GAZ_00020004"/>
        <obo:RO_0001025 rdf:resource="http://purl.obolibrary.org/obo/GAZ_00280523"/>
        <obo:IAO_0000115>A fjord in Iceland.</obo:IAO_0000115>
        <oboInOwl:hasOBONamespace>GAZ</oboInOwl:hasOBONamespace>
        <oboInOwl:id>GAZ:00145776</oboInOwl:id>
        <rdfs:label>Faskrudsfjoerdur</rdfs:label>
    </owl:NamedIndividual>
    


    <!-- http://purl.obolibrary.org/obo/GAZ_00145778 -->

    <owl:NamedIndividual rdf:about="http://purl.obolibrary.org/obo/GAZ_00145778">
        <obo:RO_0001025 rdf:resource="http://purl.obolibrary.org/obo/GAZ_00020006"/>
        <obo:RO_0001025 rdf:resource="http://purl.obolibrary.org/obo/GAZ_00280522"/>
        <obo:IAO_0000115>A bay in eastern Iceland, formed by the outflowing of the Jokulsa river.</obo:IAO_0000115>
        <oboInOwl:hasOBONamespace>GAZ</oboInOwl:hasOBONamespace>
        <oboInOwl:id>GAZ:00145778</oboInOwl:id>
        <rdfs:label>Heradsfloi</rdfs:label>
    </owl:NamedIndividual>
    


    <!-- http://purl.obolibrary.org/obo/GAZ_00145779 -->

    <owl:NamedIndividual rdf:about="http://purl.obolibrary.org/obo/GAZ_00145779">
        <obo:RO_0001025 rdf:resource="http://purl.obolibrary.org/obo/GAZ_00145764"/>
        <obo:RO_0001025 rdf:resource="http://purl.obolibrary.org/obo/GAZ_00280523"/>
        <obo:IAO_0000115>A fjord in Iceland.</obo:IAO_0000115>
        <oboInOwl:hasOBONamespace>GAZ</oboInOwl:hasOBONamespace>
        <oboInOwl:id>GAZ:00145779</oboInOwl:id>
        <rdfs:label>Kollafjoerdur [WestfjordsS]</rdfs:label>
    </owl:NamedIndividual>
    


    <!-- http://purl.obolibrary.org/obo/GAZ_00145780 -->

    <owl:NamedIndividual rdf:about="http://purl.obolibrary.org/obo/GAZ_00145780">
        <obo:RO_0001025 rdf:resource="http://purl.obolibrary.org/obo/GAZ_00020008"/>
        <obo:RO_0001025 rdf:resource="http://purl.obolibrary.org/obo/GAZ_00280523"/>
        <obo:IAO_0000115>A small fjord in southeastern Iceland. The town Hofn is located on its shores.</obo:IAO_0000115>
        <oboInOwl:hasOBONamespace>GAZ</oboInOwl:hasOBONamespace>
        <oboInOwl:id>GAZ:00145780</oboInOwl:id>
        <rdfs:label>Hornafjoerdur</rdfs:label>
    </owl:NamedIndividual>
    


    <!-- http://purl.obolibrary.org/obo/GAZ_00145782 -->

    <owl:NamedIndividual rdf:about="http://purl.obolibrary.org/obo/GAZ_00145782">
        <obo:RO_0001025 rdf:resource="http://purl.obolibrary.org/obo/GAZ_00001207"/>
        <obo:RO_0001025 rdf:resource="http://purl.obolibrary.org/obo/GAZ_00280522"/>
        <obo:IAO_0000115>A fjord in N Iceland.</obo:IAO_0000115>
        <oboInOwl:hasOBONamespace>GAZ</oboInOwl:hasOBONamespace>
        <oboInOwl:id>GAZ:00145782</oboInOwl:id>
        <rdfs:label>Siglufjoerdur</rdfs:label>
    </owl:NamedIndividual>
    


    <!-- http://purl.obolibrary.org/obo/GAZ_00145783 -->

    <owl:NamedIndividual rdf:about="http://purl.obolibrary.org/obo/GAZ_00145783">
        <obo:RO_0001025 rdf:resource="http://purl.obolibrary.org/obo/GAZ_00001203"/>
        <obo:RO_0001025 rdf:resource="http://purl.obolibrary.org/obo/GAZ_00280522"/>
        <obo:IAO_0000115>A fjord in E Iceland.</obo:IAO_0000115>
        <oboInOwl:hasOBONamespace>GAZ</oboInOwl:hasOBONamespace>
        <oboInOwl:id>GAZ:00145783</oboInOwl:id>
        <rdfs:label>Mjoifjoerdur [East]</rdfs:label>
    </owl:NamedIndividual>
    


    <!-- http://purl.obolibrary.org/obo/GAZ_00145784 -->

    <owl:NamedIndividual rdf:about="http://purl.obolibrary.org/obo/GAZ_00145784">
        <obo:RO_0001025 rdf:resource="http://purl.obolibrary.org/obo/GAZ_00280523"/>
        <obo:IAO_0000115>A large fjord in the Westfjords region of Iceland. It is 30 km long and f5 to 10 km wide.</obo:IAO_0000115>
        <oboInOwl:hasOBONamespace>GAZ</oboInOwl:hasOBONamespace>
        <oboInOwl:id>GAZ:00145784</oboInOwl:id>
        <rdfs:label>Arnarfjoerdur</rdfs:label>
    </owl:NamedIndividual>
    


    <!-- http://purl.obolibrary.org/obo/GAZ_00145785 -->

    <owl:NamedIndividual rdf:about="http://purl.obolibrary.org/obo/GAZ_00145785">
        <obo:RO_0001025 rdf:resource="http://purl.obolibrary.org/obo/GAZ_00001202"/>
        <obo:RO_0001025 rdf:resource="http://purl.obolibrary.org/obo/GAZ_00280522"/>
        <obo:IAO_0000115>A small fjord in the northwest of Iceland. It is fed by the river Austura, is roughly 2 km wide and 10 km long, and empties onto Hunafloi bay.</obo:IAO_0000115>
        <oboInOwl:hasOBONamespace>GAZ</oboInOwl:hasOBONamespace>
        <oboInOwl:id>GAZ:00145785</oboInOwl:id>
        <rdfs:label>Midfjoerdur [NW]</rdfs:label>
    </owl:NamedIndividual>
    


    <!-- http://purl.obolibrary.org/obo/GAZ_00145786 -->

    <owl:NamedIndividual rdf:about="http://purl.obolibrary.org/obo/GAZ_00145786">
        <obo:RO_0001025 rdf:resource="http://purl.obolibrary.org/obo/GAZ_00001207"/>
        <obo:RO_0001025 rdf:resource="http://purl.obolibrary.org/obo/GAZ_00280522"/>
        <obo:IAO_0000115>A fjord in northeast Iceland, near the town Thorshofn. Between the Langanes and Melrakkasletta peninsulas.</obo:IAO_0000115>
        <oboInOwl:hasOBONamespace>GAZ</oboInOwl:hasOBONamespace>
        <oboInOwl:id>GAZ:00145786</oboInOwl:id>
        <rdfs:label>Thistilfjoerdur</rdfs:label>
    </owl:NamedIndividual>
    


    <!-- http://purl.obolibrary.org/obo/GAZ_00145787 -->

    <owl:NamedIndividual rdf:about="http://purl.obolibrary.org/obo/GAZ_00145787">
        <obo:RO_0001025 rdf:resource="http://purl.obolibrary.org/obo/GAZ_00001203"/>
        <obo:RO_0001025 rdf:resource="http://purl.obolibrary.org/obo/GAZ_00020004"/>
        <obo:RO_0001025 rdf:resource="http://purl.obolibrary.org/obo/GAZ_00280523"/>
        <obo:IAO_0000115>A fjord in E Iceland.</obo:IAO_0000115>
        <oboInOwl:hasOBONamespace>GAZ</oboInOwl:hasOBONamespace>
        <oboInOwl:id>GAZ:00145787</oboInOwl:id>
        <rdfs:label>Stoedvarfjoerdur</rdfs:label>
    </owl:NamedIndividual>
    


    <!-- http://purl.obolibrary.org/obo/GAZ_00145788 -->

    <owl:NamedIndividual rdf:about="http://purl.obolibrary.org/obo/GAZ_00145788">
        <rdf:type rdf:resource="http://purl.obolibrary.org/obo/ENVO_00000305"/>
        <obo:RO_0001025 rdf:resource="http://purl.obolibrary.org/obo/GAZ_00001203"/>
        <obo:IAO_0000115>A headland on the southeastern Icelandic coast, near Hofn and Hornafjoerdur.</obo:IAO_0000115>
        <oboInOwl:hasOBONamespace>GAZ</oboInOwl:hasOBONamespace>
        <oboInOwl:id>GAZ:00145788</oboInOwl:id>
        <rdfs:label>Stokksnes</rdfs:label>
    </owl:NamedIndividual>
    


    <!-- http://purl.obolibrary.org/obo/GAZ_00145789 -->

    <owl:NamedIndividual rdf:about="http://purl.obolibrary.org/obo/GAZ_00145789">
        <obo:RO_0001025 rdf:resource="http://purl.obolibrary.org/obo/GAZ_00001206"/>
        <obo:IAO_0000115>The valley of the river Reykjadalsa.</obo:IAO_0000115>
        <oboInOwl:hasOBONamespace>GAZ</oboInOwl:hasOBONamespace>
        <oboInOwl:id>GAZ:00145789</oboInOwl:id>
        <rdfs:label>Reykholtsdalur</rdfs:label>
    </owl:NamedIndividual>
    


    <!-- http://purl.obolibrary.org/obo/GAZ_00145790 -->

    <owl:NamedIndividual rdf:about="http://purl.obolibrary.org/obo/GAZ_00145790">
        <obo:RO_0001025 rdf:resource="http://purl.obolibrary.org/obo/GAZ_00145789"/>
        <obo:IAO_0000115>A hotspring in Reykholtsdalur, Iceland. It is characterized by a very high flow rate for a hot spring (180 liters/second) and water emerges at 97degreesC. It is the highest-flow hot spring in Europe.</obo:IAO_0000115>
        <oboInOwl:hasOBONamespace>GAZ</oboInOwl:hasOBONamespace>
        <oboInOwl:id>GAZ:00145790</oboInOwl:id>
        <rdfs:label>Deildartunguhver</rdfs:label>
    </owl:NamedIndividual>
    


    <!-- http://purl.obolibrary.org/obo/GAZ_00145791 -->

    <owl:NamedIndividual rdf:about="http://purl.obolibrary.org/obo/GAZ_00145791">
        <obo:RO_0001025 rdf:resource="http://purl.obolibrary.org/obo/GAZ_00001207"/>
        <obo:RO_0001025 rdf:resource="http://purl.obolibrary.org/obo/GAZ_00280522"/>
        <obo:IAO_0000115>A large bay in eastern Iceland, to the north of Bakkafjoerdur.</obo:IAO_0000115>
        <oboInOwl:hasOBONamespace>GAZ</oboInOwl:hasOBONamespace>
        <oboInOwl:id>GAZ:00145791</oboInOwl:id>
        <rdfs:label>Bakkafloi</rdfs:label>
    </owl:NamedIndividual>
    


    <!-- http://purl.obolibrary.org/obo/GAZ_00145792 -->

    <owl:NamedIndividual rdf:about="http://purl.obolibrary.org/obo/GAZ_00145792">
        <obo:RO_0001025 rdf:resource="http://purl.obolibrary.org/obo/GAZ_00020032"/>
        <obo:IAO_0000115>A hot spring.</obo:IAO_0000115>
        <oboInOwl:hasOBONamespace>GAZ</oboInOwl:hasOBONamespace>
        <oboInOwl:id>GAZ:00145792</oboInOwl:id>
        <rdfs:label>Blue Lagoon</rdfs:label>
    </owl:NamedIndividual>
    


    <!-- http://purl.obolibrary.org/obo/GAZ_00145793 -->

    <owl:NamedIndividual rdf:about="http://purl.obolibrary.org/obo/GAZ_00145793">
        <obo:RO_0001025 rdf:resource="http://purl.obolibrary.org/obo/GAZ_00001208"/>
        <obo:IAO_0000115>A peninsula.</obo:IAO_0000115>
        <oboInOwl:hasOBONamespace>GAZ</oboInOwl:hasOBONamespace>
        <oboInOwl:id>GAZ:00145793</oboInOwl:id>
        <rdfs:label>Seltjarnarnes</rdfs:label>
    </owl:NamedIndividual>
    


    <!-- http://purl.obolibrary.org/obo/GAZ_00280113 -->

    <owl:NamedIndividual rdf:about="http://purl.obolibrary.org/obo/GAZ_00280113">
        <obo:RO_0001025 rdf:resource="http://purl.obolibrary.org/obo/GAZ_00053330"/>
        <obo:IAO_0000115>An active volcano. Below Eyjafjallajokull [ice cap].</obo:IAO_0000115>
        <oboInOwl:hasOBONamespace>GAZ</oboInOwl:hasOBONamespace>
        <oboInOwl:id>GAZ:00280113</oboInOwl:id>
        <rdfs:label>Eyjafjallajokull [volcano]</rdfs:label>
    </owl:NamedIndividual>
    


    <!-- http://purl.obolibrary.org/obo/GAZ_00280115 -->

    <owl:NamedIndividual rdf:about="http://purl.obolibrary.org/obo/GAZ_00280115">
        <obo:RO_0001025 rdf:resource="http://purl.obolibrary.org/obo/GAZ_00001207"/>
        <obo:IAO_0000115>An ice cap.</obo:IAO_0000115>
        <oboInOwl:hasOBONamespace>GAZ</oboInOwl:hasOBONamespace>
        <oboInOwl:id>GAZ:00280115</oboInOwl:id>
        <rdfs:label>Tungnafellsjokull [ice cap]</rdfs:label>
    </owl:NamedIndividual>
    


    <!-- http://purl.obolibrary.org/obo/GAZ_00280116 -->

    <owl:NamedIndividual rdf:about="http://purl.obolibrary.org/obo/GAZ_00280116">
        <obo:RO_0001025 rdf:resource="http://purl.obolibrary.org/obo/GAZ_00001207"/>
        <obo:IAO_0000115>A sandur. Located between the Hofsjokull and Vatnajokull ice-caps.</obo:IAO_0000115>
        <oboInOwl:hasOBONamespace>GAZ</oboInOwl:hasOBONamespace>
        <oboInOwl:id>GAZ:00280116</oboInOwl:id>
        <rdfs:label>Sprengisandur</rdfs:label>
    </owl:NamedIndividual>
    


    <!-- http://purl.obolibrary.org/obo/GAZ_00280117 -->

    <owl:NamedIndividual rdf:about="http://purl.obolibrary.org/obo/GAZ_00280117">
        <obo:RO_0001025 rdf:resource="http://purl.obolibrary.org/obo/GAZ_00001204"/>
        <obo:IAO_0000115>Iceland&apos;s longest river at 230 km. It is in the southern region of the island. It has its source on the glacier Hofsjokull. It flows out through narrow gorges in the highlands of Iceland. Then it passes by the historical farm of Stong. Further downstream, another river, the Tungnaa, flows into it before it enters the lowlands.</obo:IAO_0000115>
        <oboInOwl:hasOBONamespace>GAZ</oboInOwl:hasOBONamespace>
        <oboInOwl:id>GAZ:00280117</oboInOwl:id>
        <rdfs:label>Thjorsa</rdfs:label>
    </owl:NamedIndividual>
    


    <!-- http://purl.obolibrary.org/obo/GAZ_00280119 -->

    <owl:NamedIndividual rdf:about="http://purl.obolibrary.org/obo/GAZ_00280119">
        <obo:RO_0001025 rdf:resource="http://purl.obolibrary.org/obo/GAZ_00145764"/>
        <obo:IAO_0000115>A heath.</obo:IAO_0000115>
        <oboInOwl:hasOBONamespace>GAZ</oboInOwl:hasOBONamespace>
        <oboInOwl:id>GAZ:00280119</oboInOwl:id>
        <rdfs:label>Ofeigsfjardarheidi</rdfs:label>
    </owl:NamedIndividual>
    


    <!-- http://purl.obolibrary.org/obo/GAZ_00280124 -->

    <owl:NamedIndividual rdf:about="http://purl.obolibrary.org/obo/GAZ_00280124">
        <obo:RO_0001025 rdf:resource="http://purl.obolibrary.org/obo/GAZ_00001204"/>
        <obo:IAO_0000115>A river. It runs from Thingvallavatn for 21.9 km to its confluence with the river Hviia, forming the river Olfusa.</obo:IAO_0000115>
        <oboInOwl:hasOBONamespace>GAZ</oboInOwl:hasOBONamespace>
        <oboInOwl:id>GAZ:00280124</oboInOwl:id>
        <rdfs:label>Sog River</rdfs:label>
    </owl:NamedIndividual>
    


    <!-- http://purl.obolibrary.org/obo/GAZ_00280125 -->

    <owl:NamedIndividual rdf:about="http://purl.obolibrary.org/obo/GAZ_00280125">
        <obo:RO_0001025 rdf:resource="http://purl.obolibrary.org/obo/GAZ_00280124"/>
        <obo:IAO_0000115>A hydroelectric power station.</obo:IAO_0000115>
        <oboInOwl:hasOBONamespace>GAZ</oboInOwl:hasOBONamespace>
        <oboInOwl:id>GAZ:00280125</oboInOwl:id>
        <rdfs:label>Ljosafossstoo</rdfs:label>
    </owl:NamedIndividual>
    


    <!-- http://purl.obolibrary.org/obo/GAZ_00280126 -->

    <owl:NamedIndividual rdf:about="http://purl.obolibrary.org/obo/GAZ_00280126">
        <obo:RO_0001025 rdf:resource="http://purl.obolibrary.org/obo/GAZ_00280124"/>
        <obo:IAO_0000115>A hydroelectric power station.</obo:IAO_0000115>
        <oboInOwl:hasOBONamespace>GAZ</oboInOwl:hasOBONamespace>
        <oboInOwl:id>GAZ:00280126</oboInOwl:id>
        <rdfs:label>Irafossstoo</rdfs:label>
    </owl:NamedIndividual>
    


    <!-- http://purl.obolibrary.org/obo/GAZ_00280127 -->

    <owl:NamedIndividual rdf:about="http://purl.obolibrary.org/obo/GAZ_00280127">
        <obo:RO_0001025 rdf:resource="http://purl.obolibrary.org/obo/GAZ_00280124"/>
        <obo:IAO_0000115>A hydroelectric power station.</obo:IAO_0000115>
        <oboInOwl:hasOBONamespace>GAZ</oboInOwl:hasOBONamespace>
        <oboInOwl:id>GAZ:00280127</oboInOwl:id>
        <rdfs:label>Steingrimsstoo</rdfs:label>
    </owl:NamedIndividual>
    


    <!-- http://purl.obolibrary.org/obo/GAZ_00280128 -->

    <owl:NamedIndividual rdf:about="http://purl.obolibrary.org/obo/GAZ_00280128">
        <obo:RO_0001025 rdf:resource="http://purl.obolibrary.org/obo/GAZ_00280124"/>
        <obo:IAO_0000115>A lake.</obo:IAO_0000115>
        <oboInOwl:hasOBONamespace>GAZ</oboInOwl:hasOBONamespace>
        <oboInOwl:id>GAZ:00280128</oboInOwl:id>
        <rdfs:label>Ulfljotsvat</rdfs:label>
    </owl:NamedIndividual>
    


    <!-- http://purl.obolibrary.org/obo/GAZ_00280129 -->

    <owl:NamedIndividual rdf:about="http://purl.obolibrary.org/obo/GAZ_00280129">
        <obo:RO_0001025 rdf:resource="http://purl.obolibrary.org/obo/GAZ_00280124"/>
        <obo:IAO_0000115>A lake.</obo:IAO_0000115>
        <oboInOwl:hasOBONamespace>GAZ</oboInOwl:hasOBONamespace>
        <oboInOwl:id>GAZ:00280129</oboInOwl:id>
        <rdfs:label>Alftavatn</rdfs:label>
    </owl:NamedIndividual>
    


    <!-- http://purl.obolibrary.org/obo/GAZ_00280130 -->

    <owl:NamedIndividual rdf:about="http://purl.obolibrary.org/obo/GAZ_00280130">
        <obo:RO_0001025 rdf:resource="http://purl.obolibrary.org/obo/GAZ_00145755"/>
        <obo:IAO_0000115>An island.</obo:IAO_0000115>
        <oboInOwl:hasOBONamespace>GAZ</oboInOwl:hasOBONamespace>
        <oboInOwl:id>GAZ:00280130</oboInOwl:id>
        <rdfs:label>Vigur [Wesrfjords]</rdfs:label>
    </owl:NamedIndividual>
    


    <!-- http://purl.obolibrary.org/obo/GAZ_00280131 -->

    <owl:NamedIndividual rdf:about="http://purl.obolibrary.org/obo/GAZ_00280131">
        <obo:RO_0001025 rdf:resource="http://purl.obolibrary.org/obo/GAZ_00145755"/>
        <obo:RO_0001025 rdf:resource="http://purl.obolibrary.org/obo/GAZ_00145764"/>
        <obo:IAO_0000115>A fjord.</obo:IAO_0000115>
        <oboInOwl:hasOBONamespace>GAZ</oboInOwl:hasOBONamespace>
        <oboInOwl:id>GAZ:00280131</oboInOwl:id>
        <rdfs:label>Seydisfjoerdur [Westfjords]</rdfs:label>
    </owl:NamedIndividual>
    


    <!-- http://purl.obolibrary.org/obo/GAZ_00280132 -->

    <owl:NamedIndividual rdf:about="http://purl.obolibrary.org/obo/GAZ_00280132">
        <obo:RO_0001025 rdf:resource="http://purl.obolibrary.org/obo/GAZ_00145755"/>
        <obo:RO_0001025 rdf:resource="http://purl.obolibrary.org/obo/GAZ_00145764"/>
        <obo:IAO_0000115>A fjord.</obo:IAO_0000115>
        <oboInOwl:hasOBONamespace>GAZ</oboInOwl:hasOBONamespace>
        <oboInOwl:id>GAZ:00280132</oboInOwl:id>
        <rdfs:label>Mjoifjoerdur [Westfjords]</rdfs:label>
    </owl:NamedIndividual>
    


    <!-- http://purl.obolibrary.org/obo/GAZ_00280133 -->

    <owl:NamedIndividual rdf:about="http://purl.obolibrary.org/obo/GAZ_00280133">
        <obo:RO_0001025 rdf:resource="http://purl.obolibrary.org/obo/GAZ_00145791"/>
        <obo:IAO_0000115>A fjord.</obo:IAO_0000115>
        <oboInOwl:hasOBONamespace>GAZ</oboInOwl:hasOBONamespace>
        <oboInOwl:id>GAZ:00280133</oboInOwl:id>
        <rdfs:label>Midfjoerdur [NE]</rdfs:label>
    </owl:NamedIndividual>
    


    <!-- http://purl.obolibrary.org/obo/GAZ_00280134 -->

    <owl:NamedIndividual rdf:about="http://purl.obolibrary.org/obo/GAZ_00280134">
        <obo:RO_0001025 rdf:resource="http://purl.obolibrary.org/obo/GAZ_00001208"/>
        <obo:RO_0001025 rdf:resource="http://purl.obolibrary.org/obo/GAZ_00145754"/>
        <obo:IAO_0000115>A fjord.</obo:IAO_0000115>
        <oboInOwl:hasOBONamespace>GAZ</oboInOwl:hasOBONamespace>
        <oboInOwl:id>GAZ:00280134</oboInOwl:id>
        <rdfs:label>Kollafjoerdur [Capital]</rdfs:label>
    </owl:NamedIndividual>
    


    <!-- http://purl.obolibrary.org/obo/GAZ_00280135 -->

    <owl:NamedIndividual rdf:about="http://purl.obolibrary.org/obo/GAZ_00280135">
        <obo:RO_0001025 rdf:resource="http://purl.obolibrary.org/obo/GAZ_00145764"/>
        <obo:RO_0001025 rdf:resource="http://purl.obolibrary.org/obo/GAZ_00280522"/>
        <obo:IAO_0000115>A fjord.</obo:IAO_0000115>
        <oboInOwl:hasOBONamespace>GAZ</oboInOwl:hasOBONamespace>
        <oboInOwl:id>GAZ:00280135</oboInOwl:id>
        <rdfs:label>Kollafjoerdur [WestfjordsN]</rdfs:label>
    </owl:NamedIndividual>
    


    <!-- http://purl.obolibrary.org/obo/GAZ_00280136 -->

    <owl:NamedIndividual rdf:about="http://purl.obolibrary.org/obo/GAZ_00280136">
        <obo:RO_0001025 rdf:resource="http://purl.obolibrary.org/obo/GAZ_00001203"/>
        <obo:IAO_0000115>A river.</obo:IAO_0000115>
        <oboInOwl:hasOBONamespace>GAZ</oboInOwl:hasOBONamespace>
        <oboInOwl:id>GAZ:00280136</oboInOwl:id>
        <rdfs:label>Jokulsa a Bru</rdfs:label>
    </owl:NamedIndividual>
    


    <!-- http://purl.obolibrary.org/obo/GAZ_00280137 -->

    <owl:NamedIndividual rdf:about="http://purl.obolibrary.org/obo/GAZ_00280137">
        <obo:RO_0001025 rdf:resource="http://purl.obolibrary.org/obo/GAZ_00001207"/>
        <obo:IAO_0000115>A river. Its source is the glacier Vatnajokull. It discharges to the Arctic Sea. Jokulsa a Fjollum streams over the waterfalls Selfoss and Dettifoss, which is the strongest waterfall of Europe, and through the canyon at Joekulsargljufur National Park, which was formed by the explosion of a volcano situated directly beneath the river.</obo:IAO_0000115>
        <oboInOwl:hasOBONamespace>GAZ</oboInOwl:hasOBONamespace>
        <oboInOwl:id>GAZ:00280137</oboInOwl:id>
        <rdfs:label>Jokulsa a Fjollum</rdfs:label>
    </owl:NamedIndividual>
    


    <!-- http://purl.obolibrary.org/obo/GAZ_00280138 -->

    <owl:NamedIndividual rdf:about="http://purl.obolibrary.org/obo/GAZ_00280138">
        <obo:RO_0001025 rdf:resource="http://purl.obolibrary.org/obo/GAZ_00001206"/>
        <obo:RO_0001025 rdf:resource="http://purl.obolibrary.org/obo/GAZ_00280523"/>
        <obo:IAO_0000115>An island.</obo:IAO_0000115>
        <oboInOwl:hasOBONamespace>GAZ</oboInOwl:hasOBONamespace>
        <oboInOwl:id>GAZ:00280138</oboInOwl:id>
        <rdfs:label>Grimsey [W]</rdfs:label>
    </owl:NamedIndividual>
    


    <!-- http://purl.obolibrary.org/obo/GAZ_00280139 -->

    <owl:NamedIndividual rdf:about="http://purl.obolibrary.org/obo/GAZ_00280139">
        <obo:RO_0001025 rdf:resource="http://purl.obolibrary.org/obo/GAZ_00020055"/>
        <obo:RO_0001025 rdf:resource="http://purl.obolibrary.org/obo/GAZ_00280522"/>
        <obo:IAO_0000115>An island.</obo:IAO_0000115>
        <oboInOwl:hasOBONamespace>GAZ</oboInOwl:hasOBONamespace>
        <oboInOwl:id>GAZ:00280139</oboInOwl:id>
        <rdfs:label>Grimsey [Westfjords]</rdfs:label>
    </owl:NamedIndividual>
    


    <!-- http://purl.obolibrary.org/obo/GAZ_00280140 -->

    <owl:NamedIndividual rdf:about="http://purl.obolibrary.org/obo/GAZ_00280140">
        <obo:RO_0001025 rdf:resource="http://purl.obolibrary.org/obo/GAZ_00001203"/>
        <obo:RO_0001025 rdf:resource="http://purl.obolibrary.org/obo/GAZ_00280523"/>
        <obo:IAO_0000115>An island.</obo:IAO_0000115>
        <oboInOwl:hasOBONamespace>GAZ</oboInOwl:hasOBONamespace>
        <oboInOwl:id>GAZ:00280140</oboInOwl:id>
        <rdfs:label>Flatey [E]</rdfs:label>
    </owl:NamedIndividual>
    


    <!-- http://purl.obolibrary.org/obo/GAZ_00280141 -->

    <owl:NamedIndividual rdf:about="http://purl.obolibrary.org/obo/GAZ_00280141">
        <obo:RO_0001025 rdf:resource="http://purl.obolibrary.org/obo/GAZ_00001205"/>
        <obo:RO_0001025 rdf:resource="http://purl.obolibrary.org/obo/GAZ_00280523"/>
        <obo:IAO_0000115>An island.</obo:IAO_0000115>
        <oboInOwl:hasOBONamespace>GAZ</oboInOwl:hasOBONamespace>
        <oboInOwl:id>GAZ:00280141</oboInOwl:id>
        <rdfs:label>Flatey [Westfjords]</rdfs:label>
    </owl:NamedIndividual>
    


    <!-- http://purl.obolibrary.org/obo/GAZ_00280142 -->

    <owl:NamedIndividual rdf:about="http://purl.obolibrary.org/obo/GAZ_00280142">
        <obo:RO_0001025 rdf:resource="http://purl.obolibrary.org/obo/GAZ_00020001"/>
        <obo:RO_0001025 rdf:resource="http://purl.obolibrary.org/obo/GAZ_00280522"/>
        <obo:IAO_0000115>A fjord.</obo:IAO_0000115>
        <oboInOwl:hasOBONamespace>GAZ</oboInOwl:hasOBONamespace>
        <oboInOwl:id>GAZ:00280142</oboInOwl:id>
        <rdfs:label>Borgarfjoerdur [E]</rdfs:label>
    </owl:NamedIndividual>
    


    <!-- http://purl.obolibrary.org/obo/GAZ_00280143 -->

    <owl:NamedIndividual rdf:about="http://purl.obolibrary.org/obo/GAZ_00280143">
        <obo:RO_0001025 rdf:resource="http://purl.obolibrary.org/obo/GAZ_00008737"/>
        <obo:IAO_0000115>A river located in the Reykjavik area in the south-west of Iceland.</obo:IAO_0000115>
        <oboInOwl:hasOBONamespace>GAZ</oboInOwl:hasOBONamespace>
        <oboInOwl:id>GAZ:00280143</oboInOwl:id>
        <rdfs:label>Ellidaa</rdfs:label>
    </owl:NamedIndividual>
    


    <!-- http://purl.obolibrary.org/obo/GAZ_00280144 -->

    <owl:NamedIndividual rdf:about="http://purl.obolibrary.org/obo/GAZ_00280144">
        <obo:RO_0001025 rdf:resource="http://purl.obolibrary.org/obo/GAZ_00280523"/>
        <obo:RO_0001025 rdf:resource="http://purl.obolibrary.org/obo/GAZ_02000603"/>
        <obo:IAO_0000115>A bay.</obo:IAO_0000115>
        <oboInOwl:hasOBONamespace>GAZ</oboInOwl:hasOBONamespace>
        <oboInOwl:id>GAZ:00280144</oboInOwl:id>
        <rdfs:label>Ellidavogur</rdfs:label>
    </owl:NamedIndividual>
    


    <!-- http://purl.obolibrary.org/obo/GAZ_00280145 -->

    <owl:NamedIndividual rdf:about="http://purl.obolibrary.org/obo/GAZ_00280145">
        <obo:RO_0001025 rdf:resource="http://purl.obolibrary.org/obo/GAZ_02000603"/>
        <obo:IAO_0000115>A protected area. Established 1950.</obo:IAO_0000115>
        <oboInOwl:hasOBONamespace>GAZ</oboInOwl:hasOBONamespace>
        <oboInOwl:id>GAZ:00280145</oboInOwl:id>
        <rdfs:label>Heidmork</rdfs:label>
    </owl:NamedIndividual>
    


    <!-- http://purl.obolibrary.org/obo/GAZ_00280146 -->

    <owl:NamedIndividual rdf:about="http://purl.obolibrary.org/obo/GAZ_00280146">
        <obo:RO_0001025 rdf:resource="http://purl.obolibrary.org/obo/GAZ_00280145"/>
        <obo:IAO_0000115>Pseudocraters.</obo:IAO_0000115>
        <oboInOwl:hasOBONamespace>GAZ</oboInOwl:hasOBONamespace>
        <oboInOwl:id>GAZ:00280146</oboInOwl:id>
        <rdfs:label>Raudholar</rdfs:label>
    </owl:NamedIndividual>
    


    <!-- http://purl.obolibrary.org/obo/GAZ_00280147 -->

    <owl:NamedIndividual rdf:about="http://purl.obolibrary.org/obo/GAZ_00280147">
        <obo:RO_0001025 rdf:resource="http://purl.obolibrary.org/obo/GAZ_00001204"/>
        <obo:IAO_0000115>A river in Iceland. It is formed when the rivers Hvita and Sog combine, just north of the town of Selfoss and flows for 25 km into the Atlantic Ocean.</obo:IAO_0000115>
        <oboInOwl:hasOBONamespace>GAZ</oboInOwl:hasOBONamespace>
        <oboInOwl:id>GAZ:00280147</oboInOwl:id>
        <rdfs:label>Olfusa</rdfs:label>
    </owl:NamedIndividual>
    


    <!-- http://purl.obolibrary.org/obo/GAZ_00280148 -->

    <owl:NamedIndividual rdf:about="http://purl.obolibrary.org/obo/GAZ_00280148">
        <obo:RO_0001025 rdf:resource="http://purl.obolibrary.org/obo/GAZ_00001204"/>
        <obo:IAO_0000115>A protected area.</obo:IAO_0000115>
        <oboInOwl:hasOBONamespace>GAZ</oboInOwl:hasOBONamespace>
        <oboInOwl:id>GAZ:00280148</oboInOwl:id>
        <rdfs:label>Floi Nature Reserve</rdfs:label>
    </owl:NamedIndividual>
    


    <!-- http://purl.obolibrary.org/obo/GAZ_00280149 -->

    <owl:NamedIndividual rdf:about="http://purl.obolibrary.org/obo/GAZ_00280149">
        <obo:RO_0001025 rdf:resource="http://purl.obolibrary.org/obo/GAZ_00019998"/>
        <obo:IAO_0000115>A river. Discharges to the Atlantic Ocean.</obo:IAO_0000115>
        <oboInOwl:hasOBONamespace>GAZ</oboInOwl:hasOBONamespace>
        <oboInOwl:id>GAZ:00280149</oboInOwl:id>
        <rdfs:label>Leirvogsq</rdfs:label>
    </owl:NamedIndividual>
    


    <!-- http://purl.obolibrary.org/obo/GAZ_00280150 -->

    <owl:NamedIndividual rdf:about="http://purl.obolibrary.org/obo/GAZ_00280150">
        <obo:RO_0001025 rdf:resource="http://purl.obolibrary.org/obo/GAZ_00019998"/>
        <obo:IAO_0000115>A river. Discharges to the Atlantic Ocean.</obo:IAO_0000115>
        <oboInOwl:hasOBONamespace>GAZ</oboInOwl:hasOBONamespace>
        <oboInOwl:id>GAZ:00280150</oboInOwl:id>
        <rdfs:label>Kaldakvisl</rdfs:label>
    </owl:NamedIndividual>
    


    <!-- http://purl.obolibrary.org/obo/GAZ_00280151 -->

    <owl:NamedIndividual rdf:about="http://purl.obolibrary.org/obo/GAZ_00280151">
        <obo:RO_0001025 rdf:resource="http://purl.obolibrary.org/obo/GAZ_00019998"/>
        <obo:IAO_0000115>A river. Discharges to the Atlantic Ocean.</obo:IAO_0000115>
        <oboInOwl:hasOBONamespace>GAZ</oboInOwl:hasOBONamespace>
        <oboInOwl:id>GAZ:00280151</oboInOwl:id>
        <rdfs:label>Varma</rdfs:label>
    </owl:NamedIndividual>
    


    <!-- http://purl.obolibrary.org/obo/GAZ_00280152 -->

    <owl:NamedIndividual rdf:about="http://purl.obolibrary.org/obo/GAZ_00280152">
        <obo:RO_0001025 rdf:resource="http://purl.obolibrary.org/obo/GAZ_00001208"/>
        <obo:IAO_0000115>A peninsula.</obo:IAO_0000115>
        <oboInOwl:hasOBONamespace>GAZ</oboInOwl:hasOBONamespace>
        <oboInOwl:id>GAZ:00280152</oboInOwl:id>
        <rdfs:label>Geldinganes</rdfs:label>
    </owl:NamedIndividual>
    


    <!-- http://purl.obolibrary.org/obo/GAZ_00280153 -->

    <owl:NamedIndividual rdf:about="http://purl.obolibrary.org/obo/GAZ_00280153">
        <obo:RO_0001025 rdf:resource="http://purl.obolibrary.org/obo/GAZ_00280134"/>
        <obo:RO_0001025 rdf:resource="http://purl.obolibrary.org/obo/GAZ_00280523"/>
        <obo:IAO_0000115>An island.</obo:IAO_0000115>
        <oboInOwl:hasOBONamespace>GAZ</oboInOwl:hasOBONamespace>
        <oboInOwl:id>GAZ:00280153</oboInOwl:id>
        <rdfs:label>Akurey</rdfs:label>
    </owl:NamedIndividual>
    


    <!-- http://purl.obolibrary.org/obo/GAZ_00280154 -->

    <owl:NamedIndividual rdf:about="http://purl.obolibrary.org/obo/GAZ_00280154">
        <obo:RO_0001025 rdf:resource="http://purl.obolibrary.org/obo/GAZ_00280134"/>
        <obo:RO_0001025 rdf:resource="http://purl.obolibrary.org/obo/GAZ_00280523"/>
        <obo:IAO_0000115>An island.</obo:IAO_0000115>
        <oboInOwl:hasOBONamespace>GAZ</oboInOwl:hasOBONamespace>
        <oboInOwl:id>GAZ:00280154</oboInOwl:id>
        <rdfs:label>Orfirisey</rdfs:label>
    </owl:NamedIndividual>
    


    <!-- http://purl.obolibrary.org/obo/GAZ_00280155 -->

    <owl:NamedIndividual rdf:about="http://purl.obolibrary.org/obo/GAZ_00280155">
        <obo:RO_0001025 rdf:resource="http://purl.obolibrary.org/obo/GAZ_00001208"/>
        <obo:RO_0001025 rdf:resource="http://purl.obolibrary.org/obo/GAZ_00280523"/>
        <obo:IAO_0000115>A fjord.</obo:IAO_0000115>
        <oboInOwl:hasOBONamespace>GAZ</oboInOwl:hasOBONamespace>
        <oboInOwl:id>GAZ:00280155</oboInOwl:id>
        <rdfs:label>Skerjafjoerdur</rdfs:label>
    </owl:NamedIndividual>
    


    <!-- http://purl.obolibrary.org/obo/GAZ_00280156 -->

    <owl:NamedIndividual rdf:about="http://purl.obolibrary.org/obo/GAZ_00280156">
        <obo:RO_0001025 rdf:resource="http://purl.obolibrary.org/obo/GAZ_00008175"/>
        <obo:RO_0001025 rdf:resource="http://purl.obolibrary.org/obo/GAZ_00280523"/>
        <obo:IAO_0000115>A bay.</obo:IAO_0000115>
        <oboInOwl:hasOBONamespace>GAZ</oboInOwl:hasOBONamespace>
        <oboInOwl:id>GAZ:00280156</oboInOwl:id>
        <rdfs:label>Hafnarfjoerdur</rdfs:label>
    </owl:NamedIndividual>
    


    <!-- http://purl.obolibrary.org/obo/GAZ_00280157 -->

    <owl:NamedIndividual rdf:about="http://purl.obolibrary.org/obo/GAZ_00280157">
        <obo:RO_0001025 rdf:resource="http://purl.obolibrary.org/obo/GAZ_00008737"/>
        <obo:IAO_0000115>A suburb of Reykjavik.</obo:IAO_0000115>
        <oboInOwl:hasOBONamespace>GAZ</oboInOwl:hasOBONamespace>
        <oboInOwl:id>GAZ:00280157</oboInOwl:id>
        <rdfs:label>Vesturbaer</rdfs:label>
    </owl:NamedIndividual>
    


    <!-- http://purl.obolibrary.org/obo/GAZ_00280158 -->

    <owl:NamedIndividual rdf:about="http://purl.obolibrary.org/obo/GAZ_00280158">
        <obo:RO_0001025 rdf:resource="http://purl.obolibrary.org/obo/GAZ_00008737"/>
        <obo:IAO_0000115>A suburb of Reykjavik.</obo:IAO_0000115>
        <oboInOwl:hasOBONamespace>GAZ</oboInOwl:hasOBONamespace>
        <oboInOwl:id>GAZ:00280158</oboInOwl:id>
        <rdfs:label>Midborg</rdfs:label>
    </owl:NamedIndividual>
    


    <!-- http://purl.obolibrary.org/obo/GAZ_00280159 -->

    <owl:NamedIndividual rdf:about="http://purl.obolibrary.org/obo/GAZ_00280159">
        <obo:RO_0001025 rdf:resource="http://purl.obolibrary.org/obo/GAZ_00008737"/>
        <obo:IAO_0000115>A suburb of Reykjavik.</obo:IAO_0000115>
        <oboInOwl:hasOBONamespace>GAZ</oboInOwl:hasOBONamespace>
        <oboInOwl:id>GAZ:00280159</oboInOwl:id>
        <rdfs:label>Hlidarnar</rdfs:label>
    </owl:NamedIndividual>
    


    <!-- http://purl.obolibrary.org/obo/GAZ_00280160 -->

    <owl:NamedIndividual rdf:about="http://purl.obolibrary.org/obo/GAZ_00280160">
        <obo:RO_0001025 rdf:resource="http://purl.obolibrary.org/obo/GAZ_00008737"/>
        <obo:IAO_0000115>A suburb of Reykjavik.</obo:IAO_0000115>
        <oboInOwl:hasOBONamespace>GAZ</oboInOwl:hasOBONamespace>
        <oboInOwl:id>GAZ:00280160</oboInOwl:id>
        <rdfs:label>Laugardalur</rdfs:label>
    </owl:NamedIndividual>
    


    <!-- http://purl.obolibrary.org/obo/GAZ_00280161 -->

    <owl:NamedIndividual rdf:about="http://purl.obolibrary.org/obo/GAZ_00280161">
        <obo:RO_0001025 rdf:resource="http://purl.obolibrary.org/obo/GAZ_00008737"/>
        <obo:IAO_0000115>A suburb of Reykjavik.</obo:IAO_0000115>
        <oboInOwl:hasOBONamespace>GAZ</oboInOwl:hasOBONamespace>
        <oboInOwl:id>GAZ:00280161</oboInOwl:id>
        <rdfs:label>Haaleiti</rdfs:label>
    </owl:NamedIndividual>
    


    <!-- http://purl.obolibrary.org/obo/GAZ_00280162 -->

    <owl:NamedIndividual rdf:about="http://purl.obolibrary.org/obo/GAZ_00280162">
        <obo:RO_0001025 rdf:resource="http://purl.obolibrary.org/obo/GAZ_00008737"/>
        <obo:IAO_0000115>A suburb of Reykjavik.</obo:IAO_0000115>
        <oboInOwl:hasOBONamespace>GAZ</oboInOwl:hasOBONamespace>
        <oboInOwl:id>GAZ:00280162</oboInOwl:id>
        <rdfs:label>Breidholt</rdfs:label>
    </owl:NamedIndividual>
    


    <!-- http://purl.obolibrary.org/obo/GAZ_00280163 -->

    <owl:NamedIndividual rdf:about="http://purl.obolibrary.org/obo/GAZ_00280163">
        <obo:RO_0001025 rdf:resource="http://purl.obolibrary.org/obo/GAZ_00008737"/>
        <obo:IAO_0000115>A suburb of Reykjavik.</obo:IAO_0000115>
        <oboInOwl:hasOBONamespace>GAZ</oboInOwl:hasOBONamespace>
        <oboInOwl:id>GAZ:00280163</oboInOwl:id>
        <rdfs:label>Arbaer</rdfs:label>
    </owl:NamedIndividual>
    


    <!-- http://purl.obolibrary.org/obo/GAZ_00280164 -->

    <owl:NamedIndividual rdf:about="http://purl.obolibrary.org/obo/GAZ_00280164">
        <obo:RO_0001025 rdf:resource="http://purl.obolibrary.org/obo/GAZ_00008737"/>
        <obo:IAO_0000115>A suburb of Reykjavik.</obo:IAO_0000115>
        <oboInOwl:hasOBONamespace>GAZ</oboInOwl:hasOBONamespace>
        <oboInOwl:id>GAZ:00280164</oboInOwl:id>
        <rdfs:label>Grafarvogur</rdfs:label>
    </owl:NamedIndividual>
    


    <!-- http://purl.obolibrary.org/obo/GAZ_00280165 -->

    <owl:NamedIndividual rdf:about="http://purl.obolibrary.org/obo/GAZ_00280165">
        <obo:RO_0001025 rdf:resource="http://purl.obolibrary.org/obo/GAZ_00008737"/>
        <obo:IAO_0000115>A suburb of Reykjavik.</obo:IAO_0000115>
        <oboInOwl:hasOBONamespace>GAZ</oboInOwl:hasOBONamespace>
        <oboInOwl:id>GAZ:00280165</oboInOwl:id>
        <rdfs:label>Kjalarnes</rdfs:label>
    </owl:NamedIndividual>
    


    <!-- http://purl.obolibrary.org/obo/GAZ_00280166 -->

    <owl:NamedIndividual rdf:about="http://purl.obolibrary.org/obo/GAZ_00280166">
        <obo:RO_0001025 rdf:resource="http://purl.obolibrary.org/obo/GAZ_00008737"/>
        <obo:IAO_0000115>A suburb of Reykjavik.</obo:IAO_0000115>
        <oboInOwl:hasOBONamespace>GAZ</oboInOwl:hasOBONamespace>
        <oboInOwl:id>GAZ:00280166</oboInOwl:id>
        <rdfs:label>Ulfarsfell</rdfs:label>
    </owl:NamedIndividual>
    


    <!-- http://purl.obolibrary.org/obo/GAZ_00280167 -->

    <owl:NamedIndividual rdf:about="http://purl.obolibrary.org/obo/GAZ_00280167">
        <obo:RO_0001025 rdf:resource="http://purl.obolibrary.org/obo/GAZ_00001203"/>
        <obo:IAO_0000115>A glacier and volcano in eastern Iceland.</obo:IAO_0000115>
        <oboInOwl:hasOBONamespace>GAZ</oboInOwl:hasOBONamespace>
        <oboInOwl:id>GAZ:00280167</oboInOwl:id>
        <rdfs:label>Thrandarjokull</rdfs:label>
    </owl:NamedIndividual>
    


    <!-- http://purl.obolibrary.org/obo/GAZ_00280168 -->

    <owl:NamedIndividual rdf:about="http://purl.obolibrary.org/obo/GAZ_00280168">
        <obo:RO_0001025 rdf:resource="http://purl.obolibrary.org/obo/GAZ_00020003"/>
        <obo:RO_0001025 rdf:resource="http://purl.obolibrary.org/obo/GAZ_00280523"/>
        <obo:IAO_0000115>A fjord.</obo:IAO_0000115>
        <oboInOwl:hasOBONamespace>GAZ</oboInOwl:hasOBONamespace>
        <oboInOwl:id>GAZ:00280168</oboInOwl:id>
        <rdfs:label>Berufjoerdur[E]</rdfs:label>
    </owl:NamedIndividual>
    


    <!-- http://purl.obolibrary.org/obo/GAZ_00280169 -->

    <owl:NamedIndividual rdf:about="http://purl.obolibrary.org/obo/GAZ_00280169">
        <obo:RO_0001025 rdf:resource="http://purl.obolibrary.org/obo/GAZ_00145764"/>
        <obo:RO_0001025 rdf:resource="http://purl.obolibrary.org/obo/GAZ_00280523"/>
        <obo:IAO_0000115>A fjord.</obo:IAO_0000115>
        <oboInOwl:hasOBONamespace>GAZ</oboInOwl:hasOBONamespace>
        <oboInOwl:id>GAZ:00280169</oboInOwl:id>
        <rdfs:label>Berufjoerdur [Westfjords]</rdfs:label>
    </owl:NamedIndividual>
    


    <!-- http://purl.obolibrary.org/obo/GAZ_00280170 -->

    <owl:NamedIndividual rdf:about="http://purl.obolibrary.org/obo/GAZ_00280170">
        <obo:RO_0001025 rdf:resource="http://purl.obolibrary.org/obo/GAZ_00020003"/>
        <obo:RO_0001025 rdf:resource="http://purl.obolibrary.org/obo/GAZ_00280523"/>
        <obo:IAO_0000115>A fjord.</obo:IAO_0000115>
        <oboInOwl:hasOBONamespace>GAZ</oboInOwl:hasOBONamespace>
        <oboInOwl:id>GAZ:00280170</oboInOwl:id>
        <rdfs:label>Hamarsfjoerdur</rdfs:label>
    </owl:NamedIndividual>
    


    <!-- http://purl.obolibrary.org/obo/GAZ_00280171 -->

    <owl:NamedIndividual rdf:about="http://purl.obolibrary.org/obo/GAZ_00280171">
        <obo:RO_0001025 rdf:resource="http://purl.obolibrary.org/obo/GAZ_00020003"/>
        <obo:RO_0001025 rdf:resource="http://purl.obolibrary.org/obo/GAZ_00280523"/>
        <obo:IAO_0000115>A fjord.</obo:IAO_0000115>
        <oboInOwl:hasOBONamespace>GAZ</oboInOwl:hasOBONamespace>
        <oboInOwl:id>GAZ:00280171</oboInOwl:id>
        <rdfs:label>Alftafjoerdur [E]</rdfs:label>
    </owl:NamedIndividual>
    


    <!-- http://purl.obolibrary.org/obo/GAZ_00280172 -->

    <owl:NamedIndividual rdf:about="http://purl.obolibrary.org/obo/GAZ_00280172">
        <obo:RO_0001025 rdf:resource="http://purl.obolibrary.org/obo/GAZ_00145755"/>
        <obo:RO_0001025 rdf:resource="http://purl.obolibrary.org/obo/GAZ_00145764"/>
        <obo:IAO_0000115>A fjord.</obo:IAO_0000115>
        <oboInOwl:hasOBONamespace>GAZ</oboInOwl:hasOBONamespace>
        <oboInOwl:id>GAZ:00280172</oboInOwl:id>
        <rdfs:label>Alftafjoerdur [Westfjords]</rdfs:label>
    </owl:NamedIndividual>
    


    <!-- http://purl.obolibrary.org/obo/GAZ_00280173 -->

    <owl:NamedIndividual rdf:about="http://purl.obolibrary.org/obo/GAZ_00280173">
        <obo:RO_0001025 rdf:resource="http://purl.obolibrary.org/obo/GAZ_00001206"/>
        <obo:RO_0001025 rdf:resource="http://purl.obolibrary.org/obo/GAZ_00053333"/>
        <obo:IAO_0000115>A fjord.</obo:IAO_0000115>
        <oboInOwl:hasOBONamespace>GAZ</oboInOwl:hasOBONamespace>
        <oboInOwl:id>GAZ:00280173</oboInOwl:id>
        <rdfs:label>Alftafjoerdur [W]</rdfs:label>
    </owl:NamedIndividual>
    


    <!-- http://purl.obolibrary.org/obo/GAZ_00280174 -->

    <owl:NamedIndividual rdf:about="http://purl.obolibrary.org/obo/GAZ_00280174">
        <obo:RO_0001025 rdf:resource="http://purl.obolibrary.org/obo/GAZ_00020009"/>
        <obo:IAO_0000115>A river.</obo:IAO_0000115>
        <oboInOwl:hasOBONamespace>GAZ</oboInOwl:hasOBONamespace>
        <oboInOwl:id>GAZ:00280174</oboInOwl:id>
        <rdfs:label>Hofsa</rdfs:label>
    </owl:NamedIndividual>
    


    <!-- http://purl.obolibrary.org/obo/GAZ_00280175 -->

    <owl:NamedIndividual rdf:about="http://purl.obolibrary.org/obo/GAZ_00280175">
        <obo:RO_0001025 rdf:resource="http://purl.obolibrary.org/obo/GAZ_00020009"/>
        <obo:IAO_0000115>A river.</obo:IAO_0000115>
        <oboInOwl:hasOBONamespace>GAZ</oboInOwl:hasOBONamespace>
        <oboInOwl:id>GAZ:00280175</oboInOwl:id>
        <rdfs:label>Sela</rdfs:label>
    </owl:NamedIndividual>
    


    <!-- http://purl.obolibrary.org/obo/GAZ_00280177 -->

    <owl:NamedIndividual rdf:about="http://purl.obolibrary.org/obo/GAZ_00280177">
        <obo:RO_0001025 rdf:resource="http://purl.obolibrary.org/obo/GAZ_00001207"/>
        <obo:IAO_0000115>A peninsula.</obo:IAO_0000115>
        <oboInOwl:hasOBONamespace>GAZ</oboInOwl:hasOBONamespace>
        <oboInOwl:id>GAZ:00280177</oboInOwl:id>
        <rdfs:label>Melrakkasletta</rdfs:label>
    </owl:NamedIndividual>
    


    <!-- http://purl.obolibrary.org/obo/GAZ_00280178 -->

    <owl:NamedIndividual rdf:about="http://purl.obolibrary.org/obo/GAZ_00280178">
        <obo:RO_0001025 rdf:resource="http://purl.obolibrary.org/obo/GAZ_00020008"/>
        <obo:IAO_0000115>A lagoon.</obo:IAO_0000115>
        <oboInOwl:hasOBONamespace>GAZ</oboInOwl:hasOBONamespace>
        <oboInOwl:id>GAZ:00280178</oboInOwl:id>
        <rdfs:label>Skardsfjoerdur</rdfs:label>
    </owl:NamedIndividual>
    


    <!-- http://purl.obolibrary.org/obo/GAZ_00280179 -->

    <owl:NamedIndividual rdf:about="http://purl.obolibrary.org/obo/GAZ_00280179">
        <obo:RO_0001025 rdf:resource="http://purl.obolibrary.org/obo/GAZ_00020005"/>
        <obo:IAO_0000115>A forest.</obo:IAO_0000115>
        <oboInOwl:hasOBONamespace>GAZ</oboInOwl:hasOBONamespace>
        <oboInOwl:id>GAZ:00280179</oboInOwl:id>
        <rdfs:label>Hallormsstadarskogur</rdfs:label>
    </owl:NamedIndividual>
    


    <!-- http://purl.obolibrary.org/obo/GAZ_00280181 -->

    <owl:NamedIndividual rdf:about="http://purl.obolibrary.org/obo/GAZ_00280181">
        <obo:IAO_0000115>A sandbank. Formed where the Glera enters the sea.</obo:IAO_0000115>
        <oboInOwl:hasOBONamespace>GAZ</oboInOwl:hasOBONamespace>
        <oboInOwl:id>GAZ:00280181</oboInOwl:id>
        <rdfs:label>Oddeyri</rdfs:label>
    </owl:NamedIndividual>
    


    <!-- http://purl.obolibrary.org/obo/GAZ_00280182 -->

    <owl:NamedIndividual rdf:about="http://purl.obolibrary.org/obo/GAZ_00280182">
        <rdf:type rdf:resource="http://purl.obolibrary.org/obo/ENVO_00000856"/>
        <obo:RO_0001025 rdf:resource="http://purl.obolibrary.org/obo/GAZ_00020019"/>
        <obo:IAO_0000115>A populated place. A town in Nordurthing municipality on the north of Iceland on the shores of Skjalfandi bay.</obo:IAO_0000115>
        <oboInOwl:hasOBONamespace>GAZ</oboInOwl:hasOBONamespace>
        <oboInOwl:id>GAZ:00280182</oboInOwl:id>
        <rdfs:label>Husavik</rdfs:label>
    </owl:NamedIndividual>
    


    <!-- http://purl.obolibrary.org/obo/GAZ_00280187 -->

    <owl:NamedIndividual rdf:about="http://purl.obolibrary.org/obo/GAZ_00280187">
        <obo:RO_0001025 rdf:resource="http://purl.obolibrary.org/obo/GAZ_00020023"/>
        <obo:IAO_0000115>A waterfall.</obo:IAO_0000115>
        <oboInOwl:hasOBONamespace>GAZ</oboInOwl:hasOBONamespace>
        <oboInOwl:id>GAZ:00280187</oboInOwl:id>
        <rdfs:label>Godafoss</rdfs:label>
    </owl:NamedIndividual>
    


    <!-- http://purl.obolibrary.org/obo/GAZ_00280188 -->

    <owl:NamedIndividual rdf:about="http://purl.obolibrary.org/obo/GAZ_00280188">
        <obo:RO_0001025 rdf:resource="http://purl.obolibrary.org/obo/GAZ_00020023"/>
        <obo:IAO_0000115>A waterfall.</obo:IAO_0000115>
        <oboInOwl:hasOBONamespace>GAZ</oboInOwl:hasOBONamespace>
        <oboInOwl:id>GAZ:00280188</oboInOwl:id>
        <rdfs:label>Aldeyjarfoss</rdfs:label>
    </owl:NamedIndividual>
    


    <!-- http://purl.obolibrary.org/obo/GAZ_00280189 -->

    <owl:NamedIndividual rdf:about="http://purl.obolibrary.org/obo/GAZ_00280189">
        <obo:RO_0001025 rdf:resource="http://purl.obolibrary.org/obo/GAZ_00020023"/>
        <obo:IAO_0000115>A forest.</obo:IAO_0000115>
        <oboInOwl:hasOBONamespace>GAZ</oboInOwl:hasOBONamespace>
        <oboInOwl:id>GAZ:00280189</oboInOwl:id>
        <rdfs:label>Vaglaskogur</rdfs:label>
    </owl:NamedIndividual>
    


    <!-- http://purl.obolibrary.org/obo/GAZ_00280190 -->

    <owl:NamedIndividual rdf:about="http://purl.obolibrary.org/obo/GAZ_00280190">
        <obo:RO_0001025 rdf:resource="http://purl.obolibrary.org/obo/GAZ_00020020"/>
        <obo:IAO_0000115>A lava field.</obo:IAO_0000115>
        <oboInOwl:hasOBONamespace>GAZ</oboInOwl:hasOBONamespace>
        <oboInOwl:id>GAZ:00280190</oboInOwl:id>
        <rdfs:label>Odadahraun</rdfs:label>
    </owl:NamedIndividual>
    


    <!-- http://purl.obolibrary.org/obo/GAZ_00280191 -->

    <owl:NamedIndividual rdf:about="http://purl.obolibrary.org/obo/GAZ_00280191">
        <obo:RO_0001025 rdf:resource="http://purl.obolibrary.org/obo/GAZ_00020020"/>
        <obo:IAO_0000115>A glacier.</obo:IAO_0000115>
        <oboInOwl:hasOBONamespace>GAZ</oboInOwl:hasOBONamespace>
        <oboInOwl:id>GAZ:00280191</oboInOwl:id>
        <rdfs:label>Dyngjujokull</rdfs:label>
    </owl:NamedIndividual>
    


    <!-- http://purl.obolibrary.org/obo/GAZ_00280212 -->

    <owl:NamedIndividual rdf:about="http://purl.obolibrary.org/obo/GAZ_00280212">
        <obo:RO_0001025 rdf:resource="http://purl.obolibrary.org/obo/GAZ_00020029"/>
        <obo:IAO_0000115>A hot spring.</obo:IAO_0000115>
        <oboInOwl:hasOBONamespace>GAZ</oboInOwl:hasOBONamespace>
        <oboInOwl:id>GAZ:00280212</oboInOwl:id>
        <rdfs:label>Hveravellir</rdfs:label>
    </owl:NamedIndividual>
    


    <!-- http://purl.obolibrary.org/obo/GAZ_00280213 -->

    <owl:NamedIndividual rdf:about="http://purl.obolibrary.org/obo/GAZ_00280213">
        <obo:RO_0001025 rdf:resource="http://purl.obolibrary.org/obo/GAZ_00001202"/>
        <obo:IAO_0000115>A lava field.</obo:IAO_0000115>
        <oboInOwl:hasOBONamespace>GAZ</oboInOwl:hasOBONamespace>
        <oboInOwl:id>GAZ:00280213</oboInOwl:id>
        <rdfs:label>Kjalhraun</rdfs:label>
    </owl:NamedIndividual>
    


    <!-- http://purl.obolibrary.org/obo/GAZ_00280214 -->

    <owl:NamedIndividual rdf:about="http://purl.obolibrary.org/obo/GAZ_00280214">
        <obo:RO_0001025 rdf:resource="http://purl.obolibrary.org/obo/GAZ_00001202"/>
        <obo:IAO_0000115>A lava field.</obo:IAO_0000115>
        <oboInOwl:hasOBONamespace>GAZ</oboInOwl:hasOBONamespace>
        <oboInOwl:id>GAZ:00280214</oboInOwl:id>
        <rdfs:label>Hallmundarhraun</rdfs:label>
    </owl:NamedIndividual>
    


    <!-- http://purl.obolibrary.org/obo/GAZ_00280245 -->

    <owl:NamedIndividual rdf:about="http://purl.obolibrary.org/obo/GAZ_00280245">
        <rdf:type rdf:resource="http://purl.obolibrary.org/obo/ENVO_00000856"/>
        <obo:RO_0001025 rdf:resource="http://purl.obolibrary.org/obo/GAZ_00001218"/>
        <obo:IAO_0000115>A former municipality. Merged 2004-08-01.</obo:IAO_0000115>
        <oboInOwl:hasOBONamespace>GAZ</oboInOwl:hasOBONamespace>
        <oboInOwl:id>GAZ:00280245</oboInOwl:id>
        <rdfs:label>[Former] Hriseyjarhreppur</rdfs:label>
    </owl:NamedIndividual>
    


    <!-- http://purl.obolibrary.org/obo/GAZ_00280264 -->

    <owl:NamedIndividual rdf:about="http://purl.obolibrary.org/obo/GAZ_00280264">
        <rdf:type rdf:resource="http://purl.obolibrary.org/obo/ENVO_00000856"/>
        <obo:RO_0001025 rdf:resource="http://purl.obolibrary.org/obo/GAZ_00001202"/>
        <obo:IAO_0000115>A municipality.</obo:IAO_0000115>
        <oboInOwl:hasOBONamespace>GAZ</oboInOwl:hasOBONamespace>
        <oboInOwl:id>GAZ:00280264</oboInOwl:id>
        <rdfs:label>Sveitarfelagid Skagastrond</rdfs:label>
    </owl:NamedIndividual>
    


    <!-- http://purl.obolibrary.org/obo/GAZ_00280269 -->

    <owl:NamedIndividual rdf:about="http://purl.obolibrary.org/obo/GAZ_00280269">
        <obo:RO_0001025 rdf:resource="http://purl.obolibrary.org/obo/GAZ_00008739"/>
        <obo:IAO_0000115>A skerry.</obo:IAO_0000115>
        <oboInOwl:hasOBONamespace>GAZ</oboInOwl:hasOBONamespace>
        <oboInOwl:id>GAZ:00280269</oboInOwl:id>
        <rdfs:label>Faxasker</rdfs:label>
    </owl:NamedIndividual>
    


    <!-- http://purl.obolibrary.org/obo/GAZ_00280270 -->

    <owl:NamedIndividual rdf:about="http://purl.obolibrary.org/obo/GAZ_00280270">
        <obo:RO_0001025 rdf:resource="http://purl.obolibrary.org/obo/GAZ_00008739"/>
        <obo:IAO_0000115>A rock.</obo:IAO_0000115>
        <oboInOwl:hasOBONamespace>GAZ</oboInOwl:hasOBONamespace>
        <oboInOwl:id>GAZ:00280270</oboInOwl:id>
        <rdfs:label>Latur</rdfs:label>
    </owl:NamedIndividual>
    


    <!-- http://purl.obolibrary.org/obo/GAZ_00280271 -->

    <owl:NamedIndividual rdf:about="http://purl.obolibrary.org/obo/GAZ_00280271">
        <obo:RO_0001025 rdf:resource="http://purl.obolibrary.org/obo/GAZ_00008739"/>
        <obo:IAO_0000115>A rock.</obo:IAO_0000115>
        <oboInOwl:hasOBONamespace>GAZ</oboInOwl:hasOBONamespace>
        <oboInOwl:id>GAZ:00280271</oboInOwl:id>
        <rdfs:label>Litli Stakkur</rdfs:label>
    </owl:NamedIndividual>
    


    <!-- http://purl.obolibrary.org/obo/GAZ_00280272 -->

    <owl:NamedIndividual rdf:about="http://purl.obolibrary.org/obo/GAZ_00280272">
        <obo:RO_0001025 rdf:resource="http://purl.obolibrary.org/obo/GAZ_00008739"/>
        <obo:IAO_0000115>A rock.</obo:IAO_0000115>
        <oboInOwl:hasOBONamespace>GAZ</oboInOwl:hasOBONamespace>
        <oboInOwl:id>GAZ:00280272</oboInOwl:id>
        <rdfs:label>Stori Stakkur</rdfs:label>
    </owl:NamedIndividual>
    


    <!-- http://purl.obolibrary.org/obo/GAZ_00280274 -->

    <owl:NamedIndividual rdf:about="http://purl.obolibrary.org/obo/GAZ_00280274">
        <obo:RO_0001025 rdf:resource="http://purl.obolibrary.org/obo/GAZ_00020042"/>
        <obo:IAO_0000115>A hot spring.</obo:IAO_0000115>
        <oboInOwl:hasOBONamespace>GAZ</oboInOwl:hasOBONamespace>
        <oboInOwl:id>GAZ:00280274</oboInOwl:id>
        <rdfs:label>Sandholshver</rdfs:label>
    </owl:NamedIndividual>
    


    <!-- http://purl.obolibrary.org/obo/GAZ_00280275 -->

    <owl:NamedIndividual rdf:about="http://purl.obolibrary.org/obo/GAZ_00280275">
        <obo:RO_0001025 rdf:resource="http://purl.obolibrary.org/obo/GAZ_00020042"/>
        <obo:IAO_0000115>A geyser.</obo:IAO_0000115>
        <oboInOwl:hasOBONamespace>GAZ</oboInOwl:hasOBONamespace>
        <oboInOwl:id>GAZ:00280275</oboInOwl:id>
        <rdfs:label>Gryla</rdfs:label>
    </owl:NamedIndividual>
    


    <!-- http://purl.obolibrary.org/obo/GAZ_00280276 -->

    <owl:NamedIndividual rdf:about="http://purl.obolibrary.org/obo/GAZ_00280276">
        <obo:RO_0001025 rdf:resource="http://purl.obolibrary.org/obo/GAZ_00001204"/>
        <obo:IAO_0000115>A valley.</obo:IAO_0000115>
        <oboInOwl:hasOBONamespace>GAZ</oboInOwl:hasOBONamespace>
        <oboInOwl:id>GAZ:00280276</oboInOwl:id>
        <rdfs:label>Haukadalur</rdfs:label>
    </owl:NamedIndividual>
    


    <!-- http://purl.obolibrary.org/obo/GAZ_00280277 -->

    <owl:NamedIndividual rdf:about="http://purl.obolibrary.org/obo/GAZ_00280277">
        <obo:RO_0001025 rdf:resource="http://purl.obolibrary.org/obo/GAZ_00280276"/>
        <obo:IAO_0000115>A geyser.</obo:IAO_0000115>
        <oboInOwl:hasOBONamespace>GAZ</oboInOwl:hasOBONamespace>
        <oboInOwl:id>GAZ:00280277</oboInOwl:id>
        <rdfs:label>Strokkur</rdfs:label>
    </owl:NamedIndividual>
    


    <!-- http://purl.obolibrary.org/obo/GAZ_00280314 -->

    <owl:NamedIndividual rdf:about="http://purl.obolibrary.org/obo/GAZ_00280314">
        <obo:RO_0001025 rdf:resource="http://purl.obolibrary.org/obo/GAZ_00020052"/>
        <obo:RO_0001025 rdf:resource="http://purl.obolibrary.org/obo/GAZ_00280523"/>
        <obo:IAO_0000115>A fjord.</obo:IAO_0000115>
        <oboInOwl:hasOBONamespace>GAZ</oboInOwl:hasOBONamespace>
        <oboInOwl:id>GAZ:00280314</oboInOwl:id>
        <rdfs:label>Onundarfjoerdur</rdfs:label>
    </owl:NamedIndividual>
    


    <!-- http://purl.obolibrary.org/obo/GAZ_00280341 -->

    <owl:NamedIndividual rdf:about="http://purl.obolibrary.org/obo/GAZ_00280341">
        <obo:RO_0001025 rdf:resource="http://purl.obolibrary.org/obo/GAZ_00020068"/>
        <obo:RO_0001025 rdf:resource="http://purl.obolibrary.org/obo/GAZ_00280523"/>
        <obo:IAO_0000115>An island.</obo:IAO_0000115>
        <oboInOwl:hasOBONamespace>GAZ</oboInOwl:hasOBONamespace>
        <oboInOwl:id>GAZ:00280341</oboInOwl:id>
        <rdfs:label>Stykkid</rdfs:label>
    </owl:NamedIndividual>
    


    <!-- http://purl.obolibrary.org/obo/GAZ_00280342 -->

    <owl:NamedIndividual rdf:about="http://purl.obolibrary.org/obo/GAZ_00280342">
        <obo:RO_0001025 rdf:resource="http://purl.obolibrary.org/obo/GAZ_00020063"/>
        <obo:IAO_0000115>A lava field.</obo:IAO_0000115>
        <oboInOwl:hasOBONamespace>GAZ</oboInOwl:hasOBONamespace>
        <oboInOwl:id>GAZ:00280342</oboInOwl:id>
        <rdfs:label>Berserkjahraun</rdfs:label>
    </owl:NamedIndividual>
    


    <!-- http://purl.obolibrary.org/obo/GAZ_00280360 -->

    <owl:NamedIndividual rdf:about="http://purl.obolibrary.org/obo/GAZ_00280360">
        <obo:RO_0001025 rdf:resource="http://purl.obolibrary.org/obo/GAZ_00001207"/>
        <obo:IAO_0000115>A peninsula.</obo:IAO_0000115>
        <oboInOwl:hasOBONamespace>GAZ</oboInOwl:hasOBONamespace>
        <oboInOwl:id>GAZ:00280360</oboInOwl:id>
        <rdfs:label>Flateyjarskagi</rdfs:label>
    </owl:NamedIndividual>
    


    <!-- http://purl.obolibrary.org/obo/GAZ_00280361 -->

    <owl:NamedIndividual rdf:about="http://purl.obolibrary.org/obo/GAZ_00280361">
        <obo:RO_0001025 rdf:resource="http://purl.obolibrary.org/obo/GAZ_00280360"/>
        <obo:IAO_0000115>A valley in northern Iceland, on Flateyjarskagi peninsula. It stretches north from Fnjoskadalur valley all the way north to Skjalfandi bay. Flateyjardalur is named after the island of Flatey, which lies just off the shore.</obo:IAO_0000115>
        <oboInOwl:hasOBONamespace>GAZ</oboInOwl:hasOBONamespace>
        <oboInOwl:id>GAZ:00280361</oboInOwl:id>
        <rdfs:label>Flateyjardalur</rdfs:label>
    </owl:NamedIndividual>
    


    <!-- http://purl.obolibrary.org/obo/GAZ_00280362 -->

    <owl:NamedIndividual rdf:about="http://purl.obolibrary.org/obo/GAZ_00280362">
        <obo:RO_0001025 rdf:resource="http://purl.obolibrary.org/obo/GAZ_00001203"/>
        <obo:IAO_0000115>A valley.</obo:IAO_0000115>
        <oboInOwl:hasOBONamespace>GAZ</oboInOwl:hasOBONamespace>
        <oboInOwl:id>GAZ:00280362</oboInOwl:id>
        <rdfs:label>Fljotsdalur</rdfs:label>
    </owl:NamedIndividual>
    


    <!-- http://purl.obolibrary.org/obo/GAZ_00280363 -->

    <owl:NamedIndividual rdf:about="http://purl.obolibrary.org/obo/GAZ_00280363">
        <obo:RO_0001025 rdf:resource="http://purl.obolibrary.org/obo/GAZ_00001206"/>
        <obo:IAO_0000115>A valley in Borgarfjardarsysla. The valley lies between Reykholtdalur and Lundarreykjadalur, and through it flow the rivers Flokadalsa and Geirsa.</obo:IAO_0000115>
        <oboInOwl:hasOBONamespace>GAZ</oboInOwl:hasOBONamespace>
        <oboInOwl:id>GAZ:00280363</oboInOwl:id>
        <rdfs:label>Flokadalur</rdfs:label>
    </owl:NamedIndividual>
    


    <!-- http://purl.obolibrary.org/obo/GAZ_00280366 -->

    <owl:NamedIndividual rdf:about="http://purl.obolibrary.org/obo/GAZ_00280366">
        <obo:RO_0001025 rdf:resource="http://purl.obolibrary.org/obo/GAZ_00001202"/>
        <obo:IAO_0000115>A valley in Skagafjardarsysla.</obo:IAO_0000115>
        <oboInOwl:hasOBONamespace>GAZ</oboInOwl:hasOBONamespace>
        <oboInOwl:id>GAZ:00280366</oboInOwl:id>
        <rdfs:label>Flokadalur</rdfs:label>
    </owl:NamedIndividual>
    


    <!-- http://purl.obolibrary.org/obo/GAZ_00280368 -->

    <owl:NamedIndividual rdf:about="http://purl.obolibrary.org/obo/GAZ_00280368">
        <obo:RO_0001025 rdf:resource="http://purl.obolibrary.org/obo/GAZ_00001202"/>
        <obo:IAO_0000115>A lagoon located in the north of Iceland near Blonduos at the Hunafjoerdur.</obo:IAO_0000115>
        <oboInOwl:hasOBONamespace>GAZ</oboInOwl:hasOBONamespace>
        <oboInOwl:id>GAZ:00280368</oboInOwl:id>
        <rdfs:label>Hopsvatn</rdfs:label>
    </owl:NamedIndividual>
    


    <!-- http://purl.obolibrary.org/obo/GAZ_00280369 -->

    <owl:NamedIndividual rdf:about="http://purl.obolibrary.org/obo/GAZ_00280369">
        <obo:RO_0001025 rdf:resource="http://purl.obolibrary.org/obo/GAZ_00280276"/>
        <obo:IAO_0000115>A geyser.</obo:IAO_0000115>
        <oboInOwl:hasOBONamespace>GAZ</oboInOwl:hasOBONamespace>
        <oboInOwl:id>GAZ:00280369</oboInOwl:id>
        <rdfs:label>Litli Geysir</rdfs:label>
    </owl:NamedIndividual>
    


    <!-- http://purl.obolibrary.org/obo/GAZ_00280370 -->

    <owl:NamedIndividual rdf:about="http://purl.obolibrary.org/obo/GAZ_00280370">
        <obo:RO_0001025 rdf:resource="http://purl.obolibrary.org/obo/GAZ_00145764"/>
        <obo:IAO_0000115>A valley.</obo:IAO_0000115>
        <oboInOwl:hasOBONamespace>GAZ</oboInOwl:hasOBONamespace>
        <oboInOwl:id>GAZ:00280370</oboInOwl:id>
        <rdfs:label>Selardalur</rdfs:label>
    </owl:NamedIndividual>
    


    <!-- http://purl.obolibrary.org/obo/GAZ_00280371 -->

    <owl:NamedIndividual rdf:about="http://purl.obolibrary.org/obo/GAZ_00280371">
        <obo:RO_0001025 rdf:resource="http://purl.obolibrary.org/obo/GAZ_00001204"/>
        <obo:IAO_0000115>A valley in Arnessysla county in Iceland that lies between mount Burfell alongside the river Thjorsa to the east and mount Skridufell to the west.</obo:IAO_0000115>
        <oboInOwl:hasOBONamespace>GAZ</oboInOwl:hasOBONamespace>
        <oboInOwl:id>GAZ:00280371</oboInOwl:id>
        <rdfs:label>Thjorsardalur</rdfs:label>
    </owl:NamedIndividual>
    


    <!-- http://purl.obolibrary.org/obo/GAZ_00280372 -->

    <owl:NamedIndividual rdf:about="http://purl.obolibrary.org/obo/GAZ_00280372">
        <obo:RO_0001025 rdf:resource="http://purl.obolibrary.org/obo/GAZ_00280371"/>
        <obo:IAO_0000115>A valley.</obo:IAO_0000115>
        <oboInOwl:hasOBONamespace>GAZ</oboInOwl:hasOBONamespace>
        <oboInOwl:id>GAZ:00280372</oboInOwl:id>
        <rdfs:label>Bergolfsstadaa</rdfs:label>
    </owl:NamedIndividual>
    


    <!-- http://purl.obolibrary.org/obo/GAZ_00280373 -->

    <owl:NamedIndividual rdf:about="http://purl.obolibrary.org/obo/GAZ_00280373">
        <obo:RO_0001025 rdf:resource="http://purl.obolibrary.org/obo/GAZ_00280371"/>
        <obo:IAO_0000115>A valley.</obo:IAO_0000115>
        <oboInOwl:hasOBONamespace>GAZ</oboInOwl:hasOBONamespace>
        <oboInOwl:id>GAZ:00280373</oboInOwl:id>
        <rdfs:label>Raudukamba</rdfs:label>
    </owl:NamedIndividual>
    


    <!-- http://purl.obolibrary.org/obo/GAZ_00280374 -->

    <owl:NamedIndividual rdf:about="http://purl.obolibrary.org/obo/GAZ_00280374">
        <obo:RO_0001025 rdf:resource="http://purl.obolibrary.org/obo/GAZ_00001204"/>
        <obo:IAO_0000115>A river in the south of Iceland. It is approximately 100 km long. It rises in the Raudafossafjoll massif, east of the volcano Hekla. The main sources for the river are the glaciers Myrdalsjokull and Eyjafjallajokull. It flows through narrow gorges in the mountainous area between the glaciers Tindfjallajokull and Torfajokull, then spreads in the wide sandur plains at Iceland&apos;s south coast, near Thorsmork. The Markarfljot takes its course first north, then west of Thorsmork and finally empties into the Atlantic west of Eyjafjallajokull.</obo:IAO_0000115>
        <oboInOwl:hasOBONamespace>GAZ</oboInOwl:hasOBONamespace>
        <oboInOwl:id>GAZ:00280374</oboInOwl:id>
        <rdfs:label>Markarfljot</rdfs:label>
    </owl:NamedIndividual>
    


    <!-- http://purl.obolibrary.org/obo/GAZ_00280377 -->

    <owl:NamedIndividual rdf:about="http://purl.obolibrary.org/obo/GAZ_00280377">
        <obo:RO_0001025 rdf:resource="http://purl.obolibrary.org/obo/GAZ_00001204"/>
        <obo:IAO_0000115>A peninsula. Located on the south coast of Iceland, not far from Vik i Myrdal. It was formerly an island of volcanic origin.</obo:IAO_0000115>
        <oboInOwl:hasOBONamespace>GAZ</oboInOwl:hasOBONamespace>
        <oboInOwl:id>GAZ:00280377</oboInOwl:id>
        <rdfs:label>Dyrholaey</rdfs:label>
    </owl:NamedIndividual>
    


    <!-- http://purl.obolibrary.org/obo/GAZ_00280378 -->

    <owl:NamedIndividual rdf:about="http://purl.obolibrary.org/obo/GAZ_00280378">
        <obo:RO_0001025 rdf:resource="http://purl.obolibrary.org/obo/GAZ_00020045"/>
        <obo:IAO_0000115>A populated place.</obo:IAO_0000115>
        <oboInOwl:hasOBONamespace>GAZ</oboInOwl:hasOBONamespace>
        <oboInOwl:id>GAZ:00280378</oboInOwl:id>
        <rdfs:label>Landsveit</rdfs:label>
    </owl:NamedIndividual>
    


    <!-- http://purl.obolibrary.org/obo/GAZ_00280379 -->

    <owl:NamedIndividual rdf:about="http://purl.obolibrary.org/obo/GAZ_00280379">
        <obo:RO_0001025 rdf:resource="http://purl.obolibrary.org/obo/GAZ_00280378"/>
        <obo:IAO_0000115>A cave. A man-made or artificial cave in Iceland. It is located in Landsveit, South Iceland. The cave is almost 50m long and the walls are covered with engravings. Its age is unknown but it is most probably from 12th or 13th century.</obo:IAO_0000115>
        <oboInOwl:hasOBONamespace>GAZ</oboInOwl:hasOBONamespace>
        <oboInOwl:id>GAZ:00280379</oboInOwl:id>
        <rdfs:label>Hellnahellir</rdfs:label>
    </owl:NamedIndividual>
    


    <!-- http://purl.obolibrary.org/obo/GAZ_00280380 -->

    <owl:NamedIndividual rdf:about="http://purl.obolibrary.org/obo/GAZ_00280380">
        <obo:RO_0001025 rdf:resource="http://purl.obolibrary.org/obo/GAZ_00280214"/>
        <obo:IAO_0000115>A lava cave. Located in western Iceland, around 60km from the settlement of Borgarnes.</obo:IAO_0000115>
        <oboInOwl:hasOBONamespace>GAZ</oboInOwl:hasOBONamespace>
        <oboInOwl:id>GAZ:00280380</oboInOwl:id>
        <rdfs:label>Surtshellir</rdfs:label>
    </owl:NamedIndividual>
    


    <!-- http://purl.obolibrary.org/obo/GAZ_00280381 -->

    <owl:NamedIndividual rdf:about="http://purl.obolibrary.org/obo/GAZ_00280381">
        <obo:RO_0001025 rdf:resource="http://purl.obolibrary.org/obo/GAZ_00280214"/>
        <obo:IAO_0000115>A lava cave.</obo:IAO_0000115>
        <oboInOwl:hasOBONamespace>GAZ</oboInOwl:hasOBONamespace>
        <oboInOwl:id>GAZ:00280381</oboInOwl:id>
        <rdfs:label>Vidgelmir</rdfs:label>
    </owl:NamedIndividual>
    


    <!-- http://purl.obolibrary.org/obo/GAZ_00280382 -->

    <owl:NamedIndividual rdf:about="http://purl.obolibrary.org/obo/GAZ_00280382">
        <obo:RO_0001025 rdf:resource="http://purl.obolibrary.org/obo/GAZ_00280214"/>
        <obo:IAO_0000115>A lava cave.</obo:IAO_0000115>
        <oboInOwl:hasOBONamespace>GAZ</oboInOwl:hasOBONamespace>
        <oboInOwl:id>GAZ:00280382</oboInOwl:id>
        <rdfs:label>Stefanshellir</rdfs:label>
    </owl:NamedIndividual>
    


    <!-- http://purl.obolibrary.org/obo/GAZ_00280383 -->

    <owl:NamedIndividual rdf:about="http://purl.obolibrary.org/obo/GAZ_00280383">
        <obo:RO_0001025 rdf:resource="http://purl.obolibrary.org/obo/GAZ_00001207"/>
        <obo:IAO_0000115>A lava cave. Sie liegt ostlich von Reykjahlid am Myvatn.</obo:IAO_0000115>
        <oboInOwl:hasOBONamespace>GAZ</oboInOwl:hasOBONamespace>
        <oboInOwl:id>GAZ:00280383</oboInOwl:id>
        <rdfs:label>Grjotagja</rdfs:label>
    </owl:NamedIndividual>
    


    <!-- http://purl.obolibrary.org/obo/GAZ_00280384 -->

    <owl:NamedIndividual rdf:about="http://purl.obolibrary.org/obo/GAZ_00280384">
        <obo:RO_0001025 rdf:resource="http://purl.obolibrary.org/obo/GAZ_00053320"/>
        <obo:IAO_0000115>A lava cave.</obo:IAO_0000115>
        <oboInOwl:hasOBONamespace>GAZ</oboInOwl:hasOBONamespace>
        <oboInOwl:id>GAZ:00280384</oboInOwl:id>
        <rdfs:label>Lofthellir</rdfs:label>
    </owl:NamedIndividual>
    


    <!-- http://purl.obolibrary.org/obo/GAZ_00280385 -->

    <owl:NamedIndividual rdf:about="http://purl.obolibrary.org/obo/GAZ_00280385">
        <obo:RO_0001025 rdf:resource="http://purl.obolibrary.org/obo/GAZ_00001204"/>
        <obo:IAO_0000115>A lava cave.</obo:IAO_0000115>
        <oboInOwl:hasOBONamespace>GAZ</oboInOwl:hasOBONamespace>
        <oboInOwl:id>GAZ:00280385</oboInOwl:id>
        <rdfs:label>Raufarholshellir</rdfs:label>
    </owl:NamedIndividual>
    


    <!-- http://purl.obolibrary.org/obo/GAZ_00280386 -->

    <owl:NamedIndividual rdf:about="http://purl.obolibrary.org/obo/GAZ_00280386">
        <obo:RO_0001025 rdf:resource="http://purl.obolibrary.org/obo/GAZ_00001207"/>
        <obo:IAO_0000115>A lava cave.</obo:IAO_0000115>
        <oboInOwl:hasOBONamespace>GAZ</oboInOwl:hasOBONamespace>
        <oboInOwl:id>GAZ:00280386</oboInOwl:id>
        <rdfs:label>Storagja</rdfs:label>
    </owl:NamedIndividual>
    


    <!-- http://purl.obolibrary.org/obo/GAZ_00280387 -->

    <owl:NamedIndividual rdf:about="http://purl.obolibrary.org/obo/GAZ_00280387">
        <obo:RO_0001025 rdf:resource="http://purl.obolibrary.org/obo/GAZ_00001204"/>
    </owl:NamedIndividual>
    


    <!-- http://purl.obolibrary.org/obo/GAZ_00280389 -->

    <owl:NamedIndividual rdf:about="http://purl.obolibrary.org/obo/GAZ_00280389">
        <obo:RO_0001025 rdf:resource="http://purl.obolibrary.org/obo/GAZ_00001203"/>
        <obo:IAO_0000115>A pensinsula. Between Seydisfjoerdur and Mjoifjoerdur.</obo:IAO_0000115>
        <oboInOwl:hasOBONamespace>GAZ</oboInOwl:hasOBONamespace>
        <oboInOwl:id>GAZ:00280389</oboInOwl:id>
        <rdfs:label>Dalatangi</rdfs:label>
    </owl:NamedIndividual>
    


    <!-- http://purl.obolibrary.org/obo/GAZ_00280390 -->

    <owl:NamedIndividual rdf:about="http://purl.obolibrary.org/obo/GAZ_00280390">
        <obo:RO_0001025 rdf:resource="http://purl.obolibrary.org/obo/GAZ_00001206"/>
        <obo:IAO_0000115>A peninsula. Between Hvalfjoerdur and Kollafjoerdur.</obo:IAO_0000115>
        <oboInOwl:hasOBONamespace>GAZ</oboInOwl:hasOBONamespace>
        <oboInOwl:id>GAZ:00280390</oboInOwl:id>
        <rdfs:label>Kjalarnes</rdfs:label>
    </owl:NamedIndividual>
    


    <!-- http://purl.obolibrary.org/obo/GAZ_00280391 -->

    <owl:NamedIndividual rdf:about="http://purl.obolibrary.org/obo/GAZ_00280391">
        <obo:RO_0001025 rdf:resource="http://purl.obolibrary.org/obo/GAZ_00001202"/>
        <obo:IAO_0000115>A peninsula. Located W of Skagafjoerdur and E of Hunafloi.</obo:IAO_0000115>
        <oboInOwl:hasOBONamespace>GAZ</oboInOwl:hasOBONamespace>
        <oboInOwl:id>GAZ:00280391</oboInOwl:id>
        <rdfs:label>Skagi</rdfs:label>
    </owl:NamedIndividual>
    


    <!-- http://purl.obolibrary.org/obo/GAZ_00280392 -->

    <owl:NamedIndividual rdf:about="http://purl.obolibrary.org/obo/GAZ_00280392">
        <obo:RO_0001025 rdf:resource="http://purl.obolibrary.org/obo/GAZ_00001202"/>
        <obo:IAO_0000115>A peninsula. Located between Midfjoerdur and Hunafloi.</obo:IAO_0000115>
        <oboInOwl:hasOBONamespace>GAZ</oboInOwl:hasOBONamespace>
        <oboInOwl:id>GAZ:00280392</oboInOwl:id>
        <rdfs:label>Vatnsnes</rdfs:label>
    </owl:NamedIndividual>
    


    <!-- http://purl.obolibrary.org/obo/GAZ_00280393 -->

    <owl:NamedIndividual rdf:about="http://purl.obolibrary.org/obo/GAZ_00280393">
        <obo:RO_0001025 rdf:resource="http://purl.obolibrary.org/obo/GAZ_00001203"/>
        <obo:IAO_0000115>A valley. Located between Egilsstadir and Reydarfjoerdur.</obo:IAO_0000115>
        <oboInOwl:hasOBONamespace>GAZ</oboInOwl:hasOBONamespace>
        <oboInOwl:id>GAZ:00280393</oboInOwl:id>
        <rdfs:label>Fagridalur</rdfs:label>
    </owl:NamedIndividual>
    


    <!-- http://purl.obolibrary.org/obo/GAZ_00280394 -->

    <owl:NamedIndividual rdf:about="http://purl.obolibrary.org/obo/GAZ_00280394">
        <obo:RO_0001025 rdf:resource="http://purl.obolibrary.org/obo/GAZ_00001204"/>
        <obo:IAO_0000115>A valley. Located 8 km W of Kirkjubaejarklaustur.</obo:IAO_0000115>
        <oboInOwl:hasOBONamespace>GAZ</oboInOwl:hasOBONamespace>
        <oboInOwl:id>GAZ:00280394</oboInOwl:id>
        <rdfs:label>Fjadrargljufur</rdfs:label>
    </owl:NamedIndividual>
    


    <!-- http://purl.obolibrary.org/obo/GAZ_00280395 -->

    <owl:NamedIndividual rdf:about="http://purl.obolibrary.org/obo/GAZ_00280395">
        <obo:RO_0001025 rdf:resource="http://purl.obolibrary.org/obo/GAZ_00001207"/>
        <obo:IAO_0000115>A valley. Located NE of Akureyri.</obo:IAO_0000115>
        <oboInOwl:hasOBONamespace>GAZ</oboInOwl:hasOBONamespace>
        <oboInOwl:id>GAZ:00280395</oboInOwl:id>
        <rdfs:label>Fnjoskadalur</rdfs:label>
    </owl:NamedIndividual>
    


    <!-- http://purl.obolibrary.org/obo/GAZ_00280396 -->

    <owl:NamedIndividual rdf:about="http://purl.obolibrary.org/obo/GAZ_00280396">
        <obo:RO_0001025 rdf:resource="http://purl.obolibrary.org/obo/GAZ_00001206"/>
        <obo:IAO_0000115>A valley.</obo:IAO_0000115>
        <oboInOwl:hasOBONamespace>GAZ</oboInOwl:hasOBONamespace>
        <oboInOwl:id>GAZ:00280396</oboInOwl:id>
        <rdfs:label>Hnappadalur</rdfs:label>
    </owl:NamedIndividual>
    


    <!-- http://purl.obolibrary.org/obo/GAZ_00280397 -->

    <owl:NamedIndividual rdf:about="http://purl.obolibrary.org/obo/GAZ_00280397">
        <obo:RO_0001025 rdf:resource="http://purl.obolibrary.org/obo/GAZ_00280396"/>
        <obo:IAO_0000115>A volcanic cone.</obo:IAO_0000115>
        <oboInOwl:hasOBONamespace>GAZ</oboInOwl:hasOBONamespace>
        <oboInOwl:id>GAZ:00280397</oboInOwl:id>
        <rdfs:label>Eldborg</rdfs:label>
    </owl:NamedIndividual>
    


    <!-- http://purl.obolibrary.org/obo/GAZ_00280398 -->

    <owl:NamedIndividual rdf:about="http://purl.obolibrary.org/obo/GAZ_00280398">
        <obo:RO_0001025 rdf:resource="http://purl.obolibrary.org/obo/GAZ_00280396"/>
        <obo:IAO_0000115>A volcanic cone.</obo:IAO_0000115>
        <oboInOwl:hasOBONamespace>GAZ</oboInOwl:hasOBONamespace>
        <oboInOwl:id>GAZ:00280398</oboInOwl:id>
        <rdfs:label>Gullborg</rdfs:label>
    </owl:NamedIndividual>
    


    <!-- http://purl.obolibrary.org/obo/GAZ_00280399 -->

    <owl:NamedIndividual rdf:about="http://purl.obolibrary.org/obo/GAZ_00280399">
        <obo:RO_0001025 rdf:resource="http://purl.obolibrary.org/obo/GAZ_00001207"/>
        <obo:IAO_0000115>A valley.</obo:IAO_0000115>
        <oboInOwl:hasOBONamespace>GAZ</oboInOwl:hasOBONamespace>
        <oboInOwl:id>GAZ:00280399</oboInOwl:id>
        <rdfs:label>Horgardalur</rdfs:label>
    </owl:NamedIndividual>
    


    <!-- http://purl.obolibrary.org/obo/GAZ_00280401 -->

    <owl:NamedIndividual rdf:about="http://purl.obolibrary.org/obo/GAZ_00280401">
        <obo:RO_0001025 rdf:resource="http://purl.obolibrary.org/obo/GAZ_00001206"/>
        <obo:IAO_0000115>A valley.</obo:IAO_0000115>
        <oboInOwl:hasOBONamespace>GAZ</oboInOwl:hasOBONamespace>
        <oboInOwl:id>GAZ:00280401</oboInOwl:id>
        <rdfs:label>Kaldidalur</rdfs:label>
    </owl:NamedIndividual>
    


    <!-- http://purl.obolibrary.org/obo/GAZ_00280402 -->

    <owl:NamedIndividual rdf:about="http://purl.obolibrary.org/obo/GAZ_00280402">
        <obo:RO_0001025 rdf:resource="http://purl.obolibrary.org/obo/GAZ_00001202"/>
        <obo:IAO_0000115>A valley.</obo:IAO_0000115>
        <oboInOwl:hasOBONamespace>GAZ</oboInOwl:hasOBONamespace>
        <oboInOwl:id>GAZ:00280402</oboInOwl:id>
        <rdfs:label>Vatnsdalur</rdfs:label>
    </owl:NamedIndividual>
    


    <!-- http://purl.obolibrary.org/obo/GAZ_00280403 -->

    <owl:NamedIndividual rdf:about="http://purl.obolibrary.org/obo/GAZ_00280403">
        <obo:RO_0001025 rdf:resource="http://purl.obolibrary.org/obo/GAZ_00053333"/>
        <obo:IAO_0000115>Islands.</obo:IAO_0000115>
        <oboInOwl:hasOBONamespace>GAZ</oboInOwl:hasOBONamespace>
        <oboInOwl:id>GAZ:00280403</oboInOwl:id>
        <rdfs:label>Bjarneyjar</rdfs:label>
    </owl:NamedIndividual>
    


    <!-- http://purl.obolibrary.org/obo/GAZ_00280404 -->

    <owl:NamedIndividual rdf:about="http://purl.obolibrary.org/obo/GAZ_00280404">
        <obo:RO_0001025 rdf:resource="http://purl.obolibrary.org/obo/GAZ_00053333"/>
        <obo:IAO_0000115>An island.</obo:IAO_0000115>
        <oboInOwl:hasOBONamespace>GAZ</oboInOwl:hasOBONamespace>
        <oboInOwl:id>GAZ:00280404</oboInOwl:id>
        <rdfs:label>Brokey</rdfs:label>
    </owl:NamedIndividual>
    


    <!-- http://purl.obolibrary.org/obo/GAZ_00280405 -->

    <owl:NamedIndividual rdf:about="http://purl.obolibrary.org/obo/GAZ_00280405">
        <obo:RO_0001025 rdf:resource="http://purl.obolibrary.org/obo/GAZ_00280523"/>
        <obo:IAO_0000115>A skerry. Located 57km SW of Reykjaness.</obo:IAO_0000115>
        <oboInOwl:hasOBONamespace>GAZ</oboInOwl:hasOBONamespace>
        <oboInOwl:id>GAZ:00280405</oboInOwl:id>
        <rdfs:label>Eldeyjarbodi</rdfs:label>
    </owl:NamedIndividual>
    


    <!-- http://purl.obolibrary.org/obo/GAZ_00280406 -->

    <owl:NamedIndividual rdf:about="http://purl.obolibrary.org/obo/GAZ_00280406">
        <obo:RO_0001025 rdf:resource="http://purl.obolibrary.org/obo/GAZ_00053333"/>
        <obo:IAO_0000115>An island.</obo:IAO_0000115>
        <oboInOwl:hasOBONamespace>GAZ</oboInOwl:hasOBONamespace>
        <oboInOwl:id>GAZ:00280406</oboInOwl:id>
        <rdfs:label>Fagurey</rdfs:label>
    </owl:NamedIndividual>
    


    <!-- http://purl.obolibrary.org/obo/GAZ_00280407 -->

    <owl:NamedIndividual rdf:about="http://purl.obolibrary.org/obo/GAZ_00280407">
        <obo:RO_0001025 rdf:resource="http://purl.obolibrary.org/obo/GAZ_00053333"/>
        <obo:IAO_0000115>An island.</obo:IAO_0000115>
        <oboInOwl:hasOBONamespace>GAZ</oboInOwl:hasOBONamespace>
        <oboInOwl:id>GAZ:00280407</oboInOwl:id>
        <rdfs:label>Bildsey</rdfs:label>
    </owl:NamedIndividual>
    


    <!-- http://purl.obolibrary.org/obo/GAZ_00280408 -->

    <owl:NamedIndividual rdf:about="http://purl.obolibrary.org/obo/GAZ_00280408">
        <obo:RO_0001025 rdf:resource="http://purl.obolibrary.org/obo/GAZ_00053333"/>
        <obo:IAO_0000115>An island.</obo:IAO_0000115>
        <oboInOwl:hasOBONamespace>GAZ</oboInOwl:hasOBONamespace>
        <oboInOwl:id>GAZ:00280408</oboInOwl:id>
        <rdfs:label>Arney</rdfs:label>
    </owl:NamedIndividual>
    


    <!-- http://purl.obolibrary.org/obo/GAZ_00280409 -->

    <owl:NamedIndividual rdf:about="http://purl.obolibrary.org/obo/GAZ_00280409">
        <obo:RO_0001025 rdf:resource="http://purl.obolibrary.org/obo/GAZ_00053333"/>
        <obo:IAO_0000115>An island.</obo:IAO_0000115>
        <oboInOwl:hasOBONamespace>GAZ</oboInOwl:hasOBONamespace>
        <oboInOwl:id>GAZ:00280409</oboInOwl:id>
        <rdfs:label>Ellidae</rdfs:label>
    </owl:NamedIndividual>
    


    <!-- http://purl.obolibrary.org/obo/GAZ_00280410 -->

    <owl:NamedIndividual rdf:about="http://purl.obolibrary.org/obo/GAZ_00280410">
        <obo:RO_0001025 rdf:resource="http://purl.obolibrary.org/obo/GAZ_00145754"/>
        <obo:IAO_0000115>An island.</obo:IAO_0000115>
        <oboInOwl:hasOBONamespace>GAZ</oboInOwl:hasOBONamespace>
        <oboInOwl:id>GAZ:00280410</oboInOwl:id>
        <rdfs:label>Hjorsey</rdfs:label>
    </owl:NamedIndividual>
    


    <!-- http://purl.obolibrary.org/obo/GAZ_00280411 -->

    <owl:NamedIndividual rdf:about="http://purl.obolibrary.org/obo/GAZ_00280411">
        <obo:RO_0001025 rdf:resource="http://purl.obolibrary.org/obo/GAZ_00053333"/>
        <obo:IAO_0000115>An island.</obo:IAO_0000115>
        <oboInOwl:hasOBONamespace>GAZ</oboInOwl:hasOBONamespace>
        <oboInOwl:id>GAZ:00280411</oboInOwl:id>
        <rdfs:label>Hoskuldsey</rdfs:label>
    </owl:NamedIndividual>
    


    <!-- http://purl.obolibrary.org/obo/GAZ_00280412 -->

    <owl:NamedIndividual rdf:about="http://purl.obolibrary.org/obo/GAZ_00280412">
        <obo:RO_0001025 rdf:resource="http://purl.obolibrary.org/obo/GAZ_00280134"/>
        <obo:IAO_0000115>An island.</obo:IAO_0000115>
        <oboInOwl:hasOBONamespace>GAZ</oboInOwl:hasOBONamespace>
        <oboInOwl:id>GAZ:00280412</oboInOwl:id>
        <rdfs:label>Lundey</rdfs:label>
    </owl:NamedIndividual>
    


    <!-- http://purl.obolibrary.org/obo/GAZ_00280413 -->

    <owl:NamedIndividual rdf:about="http://purl.obolibrary.org/obo/GAZ_00280413">
        <obo:RO_0001025 rdf:resource="http://purl.obolibrary.org/obo/GAZ_00020063"/>
        <obo:RO_0001025 rdf:resource="http://purl.obolibrary.org/obo/GAZ_00280523"/>
        <obo:IAO_0000115>An island.</obo:IAO_0000115>
        <oboInOwl:hasOBONamespace>GAZ</oboInOwl:hasOBONamespace>
        <oboInOwl:id>GAZ:00280413</oboInOwl:id>
        <rdfs:label>Melrakkaey</rdfs:label>
    </owl:NamedIndividual>
    


    <!-- http://purl.obolibrary.org/obo/GAZ_00280414 -->

    <owl:NamedIndividual rdf:about="http://purl.obolibrary.org/obo/GAZ_00280414">
        <obo:RO_0001025 rdf:resource="http://purl.obolibrary.org/obo/GAZ_00053333"/>
        <obo:IAO_0000115>An island.</obo:IAO_0000115>
        <oboInOwl:hasOBONamespace>GAZ</oboInOwl:hasOBONamespace>
        <oboInOwl:id>GAZ:00280414</oboInOwl:id>
        <rdfs:label>Oddbjarnarsker</rdfs:label>
    </owl:NamedIndividual>
    


    <!-- http://purl.obolibrary.org/obo/GAZ_00280415 -->

    <owl:NamedIndividual rdf:about="http://purl.obolibrary.org/obo/GAZ_00280415">
        <obo:RO_0001025 rdf:resource="http://purl.obolibrary.org/obo/GAZ_00145773"/>
        <obo:IAO_0000115>An island.</obo:IAO_0000115>
        <oboInOwl:hasOBONamespace>GAZ</oboInOwl:hasOBONamespace>
        <oboInOwl:id>GAZ:00280415</oboInOwl:id>
        <rdfs:label>Seley</rdfs:label>
    </owl:NamedIndividual>
    


    <!-- http://purl.obolibrary.org/obo/GAZ_00280416 -->

    <owl:NamedIndividual rdf:about="http://purl.obolibrary.org/obo/GAZ_00280416">
        <obo:RO_0001025 rdf:resource="http://purl.obolibrary.org/obo/GAZ_00145776"/>
        <obo:IAO_0000115>An island.</obo:IAO_0000115>
        <oboInOwl:hasOBONamespace>GAZ</oboInOwl:hasOBONamespace>
        <oboInOwl:id>GAZ:00280416</oboInOwl:id>
        <rdfs:label>Skrudur</rdfs:label>
    </owl:NamedIndividual>
    


    <!-- http://purl.obolibrary.org/obo/GAZ_00280417 -->

    <owl:NamedIndividual rdf:about="http://purl.obolibrary.org/obo/GAZ_00280417">
        <obo:RO_0001025 rdf:resource="http://purl.obolibrary.org/obo/GAZ_00280117"/>
        <obo:IAO_0000115>An island.</obo:IAO_0000115>
        <oboInOwl:hasOBONamespace>GAZ</oboInOwl:hasOBONamespace>
        <oboInOwl:id>GAZ:00280417</oboInOwl:id>
        <rdfs:label>Arnes</rdfs:label>
    </owl:NamedIndividual>
    


    <!-- http://purl.obolibrary.org/obo/GAZ_00280418 -->

    <owl:NamedIndividual rdf:about="http://purl.obolibrary.org/obo/GAZ_00280418">
        <obo:RO_0001025 rdf:resource="http://purl.obolibrary.org/obo/GAZ_00280134"/>
        <obo:IAO_0000115>An island.</obo:IAO_0000115>
        <oboInOwl:hasOBONamespace>GAZ</oboInOwl:hasOBONamespace>
        <oboInOwl:id>GAZ:00280418</oboInOwl:id>
        <rdfs:label>Therney</rdfs:label>
    </owl:NamedIndividual>
    


    <!-- http://purl.obolibrary.org/obo/GAZ_00280419 -->

    <owl:NamedIndividual rdf:about="http://purl.obolibrary.org/obo/GAZ_00280419">
        <obo:RO_0001025 rdf:resource="http://purl.obolibrary.org/obo/GAZ_00020038"/>
        <obo:IAO_0000115>A populated place.</obo:IAO_0000115>
        <oboInOwl:hasOBONamespace>GAZ</oboInOwl:hasOBONamespace>
        <oboInOwl:id>GAZ:00280419</oboInOwl:id>
        <rdfs:label>Reykholt</rdfs:label>
    </owl:NamedIndividual>
    


    <!-- http://purl.obolibrary.org/obo/GAZ_00280420 -->

    <owl:NamedIndividual rdf:about="http://purl.obolibrary.org/obo/GAZ_00280420">
        <obo:RO_0001025 rdf:resource="http://purl.obolibrary.org/obo/GAZ_00280419"/>
        <obo:IAO_0000115>Hot springs.</obo:IAO_0000115>
        <oboInOwl:hasOBONamespace>GAZ</oboInOwl:hasOBONamespace>
        <oboInOwl:id>GAZ:00280420</oboInOwl:id>
        <rdfs:label>Deildartunguhver</rdfs:label>
    </owl:NamedIndividual>
    


    <!-- http://purl.obolibrary.org/obo/GAZ_00280421 -->

    <owl:NamedIndividual rdf:about="http://purl.obolibrary.org/obo/GAZ_00280421">
        <obo:RO_0001025 rdf:resource="http://purl.obolibrary.org/obo/GAZ_00059062"/>
        <obo:IAO_0000115>A rift.</obo:IAO_0000115>
        <oboInOwl:hasOBONamespace>GAZ</oboInOwl:hasOBONamespace>
        <oboInOwl:id>GAZ:00280421</oboInOwl:id>
        <rdfs:label>Silfra</rdfs:label>
    </owl:NamedIndividual>
    


    <!-- http://purl.obolibrary.org/obo/GAZ_00280422 -->

    <owl:NamedIndividual rdf:about="http://purl.obolibrary.org/obo/GAZ_00280422">
        <obo:RO_0001025 rdf:resource="http://purl.obolibrary.org/obo/GAZ_00053354"/>
        <obo:IAO_0000115>A fjord.</obo:IAO_0000115>
        <oboInOwl:hasOBONamespace>GAZ</oboInOwl:hasOBONamespace>
        <oboInOwl:id>GAZ:00280422</oboInOwl:id>
        <rdfs:label>Hedinsfjoerdur</rdfs:label>
    </owl:NamedIndividual>
    


    <!-- http://purl.obolibrary.org/obo/GAZ_00280423 -->

    <owl:NamedIndividual rdf:about="http://purl.obolibrary.org/obo/GAZ_00280423">
        <obo:RO_0001025 rdf:resource="http://purl.obolibrary.org/obo/GAZ_00053354"/>
        <obo:IAO_0000115>A fjord.</obo:IAO_0000115>
        <oboInOwl:hasOBONamespace>GAZ</oboInOwl:hasOBONamespace>
        <oboInOwl:id>GAZ:00280423</oboInOwl:id>
        <rdfs:label>Olafsfjoerdur</rdfs:label>
    </owl:NamedIndividual>
    


    <!-- http://purl.obolibrary.org/obo/GAZ_00280424 -->

    <owl:NamedIndividual rdf:about="http://purl.obolibrary.org/obo/GAZ_00280424">
        <obo:RO_0001025 rdf:resource="http://purl.obolibrary.org/obo/GAZ_00001207"/>
        <obo:IAO_0000115>A peninsula.</obo:IAO_0000115>
        <oboInOwl:hasOBONamespace>GAZ</oboInOwl:hasOBONamespace>
        <oboInOwl:id>GAZ:00280424</oboInOwl:id>
        <rdfs:label>Langanes</rdfs:label>
    </owl:NamedIndividual>
    


    <!-- http://purl.obolibrary.org/obo/GAZ_00280425 -->

    <owl:NamedIndividual rdf:about="http://purl.obolibrary.org/obo/GAZ_00280425">
        <obo:RO_0001025 rdf:resource="http://purl.obolibrary.org/obo/GAZ_00145758"/>
        <obo:IAO_0000115>A fjord.</obo:IAO_0000115>
        <oboInOwl:hasOBONamespace>GAZ</oboInOwl:hasOBONamespace>
        <oboInOwl:id>GAZ:00280425</oboInOwl:id>
        <rdfs:label>Hrutafjoerdur</rdfs:label>
    </owl:NamedIndividual>
    


    <!-- http://purl.obolibrary.org/obo/GAZ_00280426 -->

    <owl:NamedIndividual rdf:about="http://purl.obolibrary.org/obo/GAZ_00280426">
        <obo:RO_0001025 rdf:resource="http://purl.obolibrary.org/obo/GAZ_00145758"/>
        <obo:IAO_0000115>A fjord.</obo:IAO_0000115>
        <oboInOwl:hasOBONamespace>GAZ</oboInOwl:hasOBONamespace>
        <oboInOwl:id>GAZ:00280426</oboInOwl:id>
        <rdfs:label>Midfjoerdur</rdfs:label>
    </owl:NamedIndividual>
    


    <!-- http://purl.obolibrary.org/obo/GAZ_00280427 -->

    <owl:NamedIndividual rdf:about="http://purl.obolibrary.org/obo/GAZ_00280427">
        <obo:RO_0001025 rdf:resource="http://purl.obolibrary.org/obo/GAZ_00145758"/>
        <obo:IAO_0000115>A fjord.</obo:IAO_0000115>
        <oboInOwl:hasOBONamespace>GAZ</oboInOwl:hasOBONamespace>
        <oboInOwl:id>GAZ:00280427</oboInOwl:id>
        <rdfs:label>Hunafjoerdur</rdfs:label>
    </owl:NamedIndividual>
    


    <!-- http://purl.obolibrary.org/obo/GAZ_00280430 -->

    <owl:NamedIndividual rdf:about="http://purl.obolibrary.org/obo/GAZ_00280430">
        <obo:RO_0001025 rdf:resource="http://purl.obolibrary.org/obo/GAZ_00020002"/>
        <obo:IAO_0000115>A bay.</obo:IAO_0000115>
        <oboInOwl:hasOBONamespace>GAZ</oboInOwl:hasOBONamespace>
        <oboInOwl:id>GAZ:00280430</oboInOwl:id>
        <rdfs:label>Breiddalsvik</rdfs:label>
    </owl:NamedIndividual>
    


    <!-- http://purl.obolibrary.org/obo/GAZ_00280431 -->

    <owl:NamedIndividual rdf:about="http://purl.obolibrary.org/obo/GAZ_00280431">
        <obo:RO_0001025 rdf:resource="http://purl.obolibrary.org/obo/GAZ_00020008"/>
        <obo:IAO_0000115>A bay.</obo:IAO_0000115>
        <oboInOwl:hasOBONamespace>GAZ</oboInOwl:hasOBONamespace>
        <oboInOwl:id>GAZ:00280431</oboInOwl:id>
        <rdfs:label>Lonsvik</rdfs:label>
    </owl:NamedIndividual>
    


    <!-- http://purl.obolibrary.org/obo/GAZ_00280432 -->

    <owl:NamedIndividual rdf:about="http://purl.obolibrary.org/obo/GAZ_00280432">
        <obo:RO_0001025 rdf:resource="http://purl.obolibrary.org/obo/GAZ_00280431"/>
        <obo:IAO_0000115>A lagoon.</obo:IAO_0000115>
        <oboInOwl:hasOBONamespace>GAZ</oboInOwl:hasOBONamespace>
        <oboInOwl:id>GAZ:00280432</oboInOwl:id>
        <rdfs:label>Lonsfjoerdur</rdfs:label>
    </owl:NamedIndividual>
    


    <!-- http://purl.obolibrary.org/obo/GAZ_00280433 -->

    <owl:NamedIndividual rdf:about="http://purl.obolibrary.org/obo/GAZ_00280433">
        <obo:RO_0001025 rdf:resource="http://purl.obolibrary.org/obo/GAZ_00280431"/>
        <obo:IAO_0000115>A lagoon.</obo:IAO_0000115>
        <oboInOwl:hasOBONamespace>GAZ</oboInOwl:hasOBONamespace>
        <oboInOwl:id>GAZ:00280433</oboInOwl:id>
        <rdfs:label>Papafjoerdur</rdfs:label>
    </owl:NamedIndividual>
    


    <!-- http://purl.obolibrary.org/obo/GAZ_00280434 -->

    <owl:NamedIndividual rdf:about="http://purl.obolibrary.org/obo/GAZ_00280434">
        <obo:RO_0001025 rdf:resource="http://purl.obolibrary.org/obo/GAZ_00145773"/>
        <obo:RO_0001025 rdf:resource="http://purl.obolibrary.org/obo/GAZ_00280522"/>
        <obo:IAO_0000115>A fjord in Iceland.</obo:IAO_0000115>
        <oboInOwl:hasOBONamespace>GAZ</oboInOwl:hasOBONamespace>
        <oboInOwl:id>GAZ:00280434</oboInOwl:id>
        <rdfs:label>Eskifjoerdur</rdfs:label>
    </owl:NamedIndividual>
    


    <!-- http://purl.obolibrary.org/obo/GAZ_00280435 -->

    <owl:NamedIndividual rdf:about="http://purl.obolibrary.org/obo/GAZ_00280435">
        <obo:RO_0001025 rdf:resource="http://purl.obolibrary.org/obo/GAZ_00020004"/>
        <obo:RO_0001025 rdf:resource="http://purl.obolibrary.org/obo/GAZ_00280522"/>
        <obo:IAO_0000115>A bay.</obo:IAO_0000115>
        <oboInOwl:hasOBONamespace>GAZ</oboInOwl:hasOBONamespace>
        <oboInOwl:id>GAZ:00280435</oboInOwl:id>
        <rdfs:label>Seydisfjardarfloi</rdfs:label>
    </owl:NamedIndividual>
    


    <!-- http://purl.obolibrary.org/obo/GAZ_00280436 -->

    <owl:NamedIndividual rdf:about="http://purl.obolibrary.org/obo/GAZ_00280436">
        <obo:RO_0001025 rdf:resource="http://purl.obolibrary.org/obo/GAZ_00280435"/>
        <obo:IAO_0000115>A fjord.</obo:IAO_0000115>
        <oboInOwl:hasOBONamespace>GAZ</oboInOwl:hasOBONamespace>
        <oboInOwl:id>GAZ:00280436</oboInOwl:id>
        <rdfs:label>Seydisfjoerdur</rdfs:label>
    </owl:NamedIndividual>
    


    <!-- http://purl.obolibrary.org/obo/GAZ_00280437 -->

    <owl:NamedIndividual rdf:about="http://purl.obolibrary.org/obo/GAZ_00280437">
        <obo:RO_0001025 rdf:resource="http://purl.obolibrary.org/obo/GAZ_00280435"/>
        <obo:IAO_0000115>A fjord.</obo:IAO_0000115>
        <oboInOwl:hasOBONamespace>GAZ</oboInOwl:hasOBONamespace>
        <oboInOwl:id>GAZ:00280437</oboInOwl:id>
        <rdfs:label>Lodmundarfjoerdur</rdfs:label>
    </owl:NamedIndividual>
    


    <!-- http://purl.obolibrary.org/obo/GAZ_00280438 -->

    <owl:NamedIndividual rdf:about="http://purl.obolibrary.org/obo/GAZ_00280438">
        <obo:RO_0001025 rdf:resource="http://purl.obolibrary.org/obo/GAZ_00145771"/>
        <obo:IAO_0000115>A fjord.</obo:IAO_0000115>
        <oboInOwl:hasOBONamespace>GAZ</oboInOwl:hasOBONamespace>
        <oboInOwl:id>GAZ:00280438</oboInOwl:id>
        <rdfs:label>Nipsfjoerdur</rdfs:label>
    </owl:NamedIndividual>
    


    <!-- http://purl.obolibrary.org/obo/GAZ_00280439 -->

    <owl:NamedIndividual rdf:about="http://purl.obolibrary.org/obo/GAZ_00280439">
        <obo:RO_0001025 rdf:resource="http://purl.obolibrary.org/obo/GAZ_00053333"/>
        <obo:IAO_0000115>A fjord.</obo:IAO_0000115>
        <oboInOwl:hasOBONamespace>GAZ</oboInOwl:hasOBONamespace>
        <oboInOwl:id>GAZ:00280439</oboInOwl:id>
        <rdfs:label>Grundarfjoerdur</rdfs:label>
    </owl:NamedIndividual>
    


    <!-- http://purl.obolibrary.org/obo/GAZ_00280440 -->

    <owl:NamedIndividual rdf:about="http://purl.obolibrary.org/obo/GAZ_00280440">
        <obo:RO_0001025 rdf:resource="http://purl.obolibrary.org/obo/GAZ_00053333"/>
        <obo:IAO_0000115>A fjord.</obo:IAO_0000115>
        <oboInOwl:hasOBONamespace>GAZ</oboInOwl:hasOBONamespace>
        <oboInOwl:id>GAZ:00280440</oboInOwl:id>
        <rdfs:label>Kolgrafafjoerdur</rdfs:label>
    </owl:NamedIndividual>
    


    <!-- http://purl.obolibrary.org/obo/GAZ_00280441 -->

    <owl:NamedIndividual rdf:about="http://purl.obolibrary.org/obo/GAZ_00280441">
        <obo:RO_0001025 rdf:resource="http://purl.obolibrary.org/obo/GAZ_00053333"/>
        <obo:IAO_0000115>A fjord.</obo:IAO_0000115>
        <oboInOwl:hasOBONamespace>GAZ</oboInOwl:hasOBONamespace>
        <oboInOwl:id>GAZ:00280441</oboInOwl:id>
        <rdfs:label>Hraunsfjoerdur</rdfs:label>
    </owl:NamedIndividual>
    


    <!-- http://purl.obolibrary.org/obo/GAZ_00280442 -->

    <owl:NamedIndividual rdf:about="http://purl.obolibrary.org/obo/GAZ_00280442">
        <obo:RO_0001025 rdf:resource="http://purl.obolibrary.org/obo/GAZ_00053333"/>
        <obo:IAO_0000115>A fjord.</obo:IAO_0000115>
        <oboInOwl:hasOBONamespace>GAZ</oboInOwl:hasOBONamespace>
        <oboInOwl:id>GAZ:00280442</oboInOwl:id>
        <rdfs:label>Gilsfjoerdur</rdfs:label>
    </owl:NamedIndividual>
    


    <!-- http://purl.obolibrary.org/obo/GAZ_00280443 -->

    <owl:NamedIndividual rdf:about="http://purl.obolibrary.org/obo/GAZ_00280443">
        <obo:RO_0001025 rdf:resource="http://purl.obolibrary.org/obo/GAZ_00053333"/>
        <obo:IAO_0000115>A fjord.</obo:IAO_0000115>
        <oboInOwl:hasOBONamespace>GAZ</oboInOwl:hasOBONamespace>
        <oboInOwl:id>GAZ:00280443</oboInOwl:id>
        <rdfs:label>Kroksfjoerdur</rdfs:label>
    </owl:NamedIndividual>
    


    <!-- http://purl.obolibrary.org/obo/GAZ_00280444 -->

    <owl:NamedIndividual rdf:about="http://purl.obolibrary.org/obo/GAZ_00280444">
        <obo:RO_0001025 rdf:resource="http://purl.obolibrary.org/obo/GAZ_00053333"/>
        <obo:IAO_0000115>A fjord.</obo:IAO_0000115>
        <oboInOwl:hasOBONamespace>GAZ</oboInOwl:hasOBONamespace>
        <oboInOwl:id>GAZ:00280444</oboInOwl:id>
        <rdfs:label>Thorskafjoerdur</rdfs:label>
    </owl:NamedIndividual>
    


    <!-- http://purl.obolibrary.org/obo/GAZ_00280445 -->

    <owl:NamedIndividual rdf:about="http://purl.obolibrary.org/obo/GAZ_00280445">
        <obo:RO_0001025 rdf:resource="http://purl.obolibrary.org/obo/GAZ_00280444"/>
        <obo:IAO_0000115>A fjord.</obo:IAO_0000115>
        <oboInOwl:hasOBONamespace>GAZ</oboInOwl:hasOBONamespace>
        <oboInOwl:id>GAZ:00280445</oboInOwl:id>
        <rdfs:label>Djupifjoerdur</rdfs:label>
    </owl:NamedIndividual>
    


    <!-- http://purl.obolibrary.org/obo/GAZ_00280446 -->

    <owl:NamedIndividual rdf:about="http://purl.obolibrary.org/obo/GAZ_00280446">
        <obo:RO_0001025 rdf:resource="http://purl.obolibrary.org/obo/GAZ_00053333"/>
        <obo:IAO_0000115>A fjord.</obo:IAO_0000115>
        <oboInOwl:hasOBONamespace>GAZ</oboInOwl:hasOBONamespace>
        <oboInOwl:id>GAZ:00280446</oboInOwl:id>
        <rdfs:label>Kvigindisfjoerdur</rdfs:label>
    </owl:NamedIndividual>
    


    <!-- http://purl.obolibrary.org/obo/GAZ_00280447 -->

    <owl:NamedIndividual rdf:about="http://purl.obolibrary.org/obo/GAZ_00280447">
        <obo:RO_0001025 rdf:resource="http://purl.obolibrary.org/obo/GAZ_00053333"/>
        <obo:IAO_0000115>A fjord.</obo:IAO_0000115>
        <oboInOwl:hasOBONamespace>GAZ</oboInOwl:hasOBONamespace>
        <oboInOwl:id>GAZ:00280447</oboInOwl:id>
        <rdfs:label>Skalmarfjoerdur</rdfs:label>
    </owl:NamedIndividual>
    


    <!-- http://purl.obolibrary.org/obo/GAZ_00280448 -->

    <owl:NamedIndividual rdf:about="http://purl.obolibrary.org/obo/GAZ_00280448">
        <obo:RO_0001025 rdf:resource="http://purl.obolibrary.org/obo/GAZ_00053333"/>
        <obo:IAO_0000115>A fjord.</obo:IAO_0000115>
        <oboInOwl:hasOBONamespace>GAZ</oboInOwl:hasOBONamespace>
        <oboInOwl:id>GAZ:00280448</oboInOwl:id>
        <rdfs:label>Kerlingarfjoerdur</rdfs:label>
    </owl:NamedIndividual>
    


    <!-- http://purl.obolibrary.org/obo/GAZ_00280449 -->

    <owl:NamedIndividual rdf:about="http://purl.obolibrary.org/obo/GAZ_00280449">
        <obo:RO_0001025 rdf:resource="http://purl.obolibrary.org/obo/GAZ_00053333"/>
        <obo:IAO_0000115>A fjord.</obo:IAO_0000115>
        <oboInOwl:hasOBONamespace>GAZ</oboInOwl:hasOBONamespace>
        <oboInOwl:id>GAZ:00280449</oboInOwl:id>
        <rdfs:label>Kjalkafjoerdur</rdfs:label>
    </owl:NamedIndividual>
    


    <!-- http://purl.obolibrary.org/obo/GAZ_00280450 -->

    <owl:NamedIndividual rdf:about="http://purl.obolibrary.org/obo/GAZ_00280450">
        <obo:RO_0001025 rdf:resource="http://purl.obolibrary.org/obo/GAZ_00053333"/>
        <obo:IAO_0000115>A fjord.</obo:IAO_0000115>
        <oboInOwl:hasOBONamespace>GAZ</oboInOwl:hasOBONamespace>
        <oboInOwl:id>GAZ:00280450</oboInOwl:id>
        <rdfs:label>Vatnsfjoerdur</rdfs:label>
    </owl:NamedIndividual>
    


    <!-- http://purl.obolibrary.org/obo/GAZ_00280451 -->

    <owl:NamedIndividual rdf:about="http://purl.obolibrary.org/obo/GAZ_00280451">
        <obo:RO_0001025 rdf:resource="http://purl.obolibrary.org/obo/GAZ_00053333"/>
        <obo:IAO_0000115>A fjord.</obo:IAO_0000115>
        <oboInOwl:hasOBONamespace>GAZ</oboInOwl:hasOBONamespace>
        <oboInOwl:id>GAZ:00280451</oboInOwl:id>
        <rdfs:label>Vigrafjoerdur</rdfs:label>
    </owl:NamedIndividual>
    


    <!-- http://purl.obolibrary.org/obo/GAZ_00280452 -->

    <owl:NamedIndividual rdf:about="http://purl.obolibrary.org/obo/GAZ_00280452">
        <obo:RO_0001025 rdf:resource="http://purl.obolibrary.org/obo/GAZ_00280444"/>
        <obo:IAO_0000115>A fjord.</obo:IAO_0000115>
        <oboInOwl:hasOBONamespace>GAZ</oboInOwl:hasOBONamespace>
        <oboInOwl:id>GAZ:00280452</oboInOwl:id>
        <rdfs:label>Gufufjoerdur</rdfs:label>
    </owl:NamedIndividual>
    


    <!-- http://purl.obolibrary.org/obo/GAZ_00280453 -->

    <owl:NamedIndividual rdf:about="http://purl.obolibrary.org/obo/GAZ_00280453">
        <obo:RO_0001025 rdf:resource="http://purl.obolibrary.org/obo/GAZ_00053333"/>
        <obo:IAO_0000115>A fjord.</obo:IAO_0000115>
        <oboInOwl:hasOBONamespace>GAZ</oboInOwl:hasOBONamespace>
        <oboInOwl:id>GAZ:00280453</oboInOwl:id>
        <rdfs:label>Kollafjprdur</rdfs:label>
    </owl:NamedIndividual>
    


    <!-- http://purl.obolibrary.org/obo/GAZ_00280454 -->

    <owl:NamedIndividual rdf:about="http://purl.obolibrary.org/obo/GAZ_00280454">
        <obo:RO_0001025 rdf:resource="http://purl.obolibrary.org/obo/GAZ_00280447"/>
        <obo:IAO_0000115>A fjord.</obo:IAO_0000115>
        <oboInOwl:hasOBONamespace>GAZ</oboInOwl:hasOBONamespace>
        <oboInOwl:id>GAZ:00280454</oboInOwl:id>
        <rdfs:label>Vattarfjoerdur</rdfs:label>
    </owl:NamedIndividual>
    


    <!-- http://purl.obolibrary.org/obo/GAZ_00280455 -->

    <owl:NamedIndividual rdf:about="http://purl.obolibrary.org/obo/GAZ_00280455">
        <obo:RO_0001025 rdf:resource="http://purl.obolibrary.org/obo/GAZ_00280448"/>
        <obo:IAO_0000115>A fjord.</obo:IAO_0000115>
        <oboInOwl:hasOBONamespace>GAZ</oboInOwl:hasOBONamespace>
        <oboInOwl:id>GAZ:00280455</oboInOwl:id>
        <rdfs:label>Mjoifjoerdur</rdfs:label>
    </owl:NamedIndividual>
    


    <!-- http://purl.obolibrary.org/obo/GAZ_00280456 -->

    <owl:NamedIndividual rdf:about="http://purl.obolibrary.org/obo/GAZ_00280456">
        <obo:RO_0001025 rdf:resource="http://purl.obolibrary.org/obo/GAZ_00020052"/>
        <obo:RO_0001025 rdf:resource="http://purl.obolibrary.org/obo/GAZ_00280523"/>
        <obo:IAO_0000115>A bay.</obo:IAO_0000115>
        <oboInOwl:hasOBONamespace>GAZ</oboInOwl:hasOBONamespace>
        <oboInOwl:id>GAZ:00280456</oboInOwl:id>
        <rdfs:label>Adalvik</rdfs:label>
    </owl:NamedIndividual>
    


    <!-- http://purl.obolibrary.org/obo/GAZ_00280457 -->

    <owl:NamedIndividual rdf:about="http://purl.obolibrary.org/obo/GAZ_00280457">
        <obo:RO_0001025 rdf:resource="http://purl.obolibrary.org/obo/GAZ_00145784"/>
        <obo:IAO_0000115>A fjord.</obo:IAO_0000115>
        <oboInOwl:hasOBONamespace>GAZ</oboInOwl:hasOBONamespace>
        <oboInOwl:id>GAZ:00280457</oboInOwl:id>
        <rdfs:label>Borgarfjoerdur</rdfs:label>
    </owl:NamedIndividual>
    


    <!-- http://purl.obolibrary.org/obo/GAZ_00280458 -->

    <owl:NamedIndividual rdf:about="http://purl.obolibrary.org/obo/GAZ_00280458">
        <obo:RO_0001025 rdf:resource="http://purl.obolibrary.org/obo/GAZ_00145784"/>
        <obo:IAO_0000115>A bay.</obo:IAO_0000115>
        <oboInOwl:hasOBONamespace>GAZ</oboInOwl:hasOBONamespace>
        <oboInOwl:id>GAZ:00280458</oboInOwl:id>
        <rdfs:label>Dynjandisvogur</rdfs:label>
    </owl:NamedIndividual>
    


    <!-- http://purl.obolibrary.org/obo/GAZ_00280459 -->

    <owl:NamedIndividual rdf:about="http://purl.obolibrary.org/obo/GAZ_00280459">
        <obo:RO_0001025 rdf:resource="http://purl.obolibrary.org/obo/GAZ_00145784"/>
        <obo:IAO_0000115>A fjord.</obo:IAO_0000115>
        <oboInOwl:hasOBONamespace>GAZ</oboInOwl:hasOBONamespace>
        <oboInOwl:id>GAZ:00280459</oboInOwl:id>
        <rdfs:label>Sudurfirdir</rdfs:label>
    </owl:NamedIndividual>
    


    <!-- http://purl.obolibrary.org/obo/GAZ_00280460 -->

    <owl:NamedIndividual rdf:about="http://purl.obolibrary.org/obo/GAZ_00280460">
        <obo:RO_0001025 rdf:resource="http://purl.obolibrary.org/obo/GAZ_00280459"/>
        <obo:IAO_0000115>A fjord.</obo:IAO_0000115>
        <oboInOwl:hasOBONamespace>GAZ</oboInOwl:hasOBONamespace>
        <oboInOwl:id>GAZ:00280460</oboInOwl:id>
        <rdfs:label>Geirthjofsfjoerdur</rdfs:label>
    </owl:NamedIndividual>
    


    <!-- http://purl.obolibrary.org/obo/GAZ_00280461 -->

    <owl:NamedIndividual rdf:about="http://purl.obolibrary.org/obo/GAZ_00280461">
        <obo:RO_0001025 rdf:resource="http://purl.obolibrary.org/obo/GAZ_00280459"/>
        <obo:IAO_0000115>A fjord.</obo:IAO_0000115>
        <oboInOwl:hasOBONamespace>GAZ</oboInOwl:hasOBONamespace>
        <oboInOwl:id>GAZ:00280461</oboInOwl:id>
        <rdfs:label>Trostansfjoerdur</rdfs:label>
    </owl:NamedIndividual>
    


    <!-- http://purl.obolibrary.org/obo/GAZ_00280462 -->

    <owl:NamedIndividual rdf:about="http://purl.obolibrary.org/obo/GAZ_00280462">
        <obo:RO_0001025 rdf:resource="http://purl.obolibrary.org/obo/GAZ_00280459"/>
        <obo:IAO_0000115>A fjord.</obo:IAO_0000115>
        <oboInOwl:hasOBONamespace>GAZ</oboInOwl:hasOBONamespace>
        <oboInOwl:id>GAZ:00280462</oboInOwl:id>
        <rdfs:label>Reykjarfjoerdur</rdfs:label>
    </owl:NamedIndividual>
    


    <!-- http://purl.obolibrary.org/obo/GAZ_00280463 -->

    <owl:NamedIndividual rdf:about="http://purl.obolibrary.org/obo/GAZ_00280463">
        <obo:RO_0001025 rdf:resource="http://purl.obolibrary.org/obo/GAZ_00280459"/>
        <obo:IAO_0000115>A fjord.</obo:IAO_0000115>
        <oboInOwl:hasOBONamespace>GAZ</oboInOwl:hasOBONamespace>
        <oboInOwl:id>GAZ:00280463</oboInOwl:id>
        <rdfs:label>Fossfjoerdur</rdfs:label>
    </owl:NamedIndividual>
    


    <!-- http://purl.obolibrary.org/obo/GAZ_00280464 -->

    <owl:NamedIndividual rdf:about="http://purl.obolibrary.org/obo/GAZ_00280464">
        <obo:RO_0001025 rdf:resource="http://purl.obolibrary.org/obo/GAZ_00145784"/>
        <obo:IAO_0000115>A bay.</obo:IAO_0000115>
        <oboInOwl:hasOBONamespace>GAZ</oboInOwl:hasOBONamespace>
        <oboInOwl:id>GAZ:00280464</oboInOwl:id>
        <rdfs:label>Bildudalsvogur</rdfs:label>
    </owl:NamedIndividual>
    


    <!-- http://purl.obolibrary.org/obo/GAZ_00280465 -->

    <owl:NamedIndividual rdf:about="http://purl.obolibrary.org/obo/GAZ_00280465">
        <obo:RO_0001025 rdf:resource="http://purl.obolibrary.org/obo/GAZ_00020052"/>
        <obo:RO_0001025 rdf:resource="http://purl.obolibrary.org/obo/GAZ_00145765"/>
        <obo:RO_0001025 rdf:resource="http://purl.obolibrary.org/obo/GAZ_00280523"/>
        <obo:IAO_0000115>A bay.</obo:IAO_0000115>
        <oboInOwl:hasOBONamespace>GAZ</oboInOwl:hasOBONamespace>
        <oboInOwl:id>GAZ:00280465</oboInOwl:id>
        <rdfs:label>Fljotavik</rdfs:label>
    </owl:NamedIndividual>
    


    <!-- http://purl.obolibrary.org/obo/GAZ_00280466 -->

    <owl:NamedIndividual rdf:about="http://purl.obolibrary.org/obo/GAZ_00280466">
        <obo:RO_0001025 rdf:resource="http://purl.obolibrary.org/obo/GAZ_00280392"/>
        <obo:RO_0001025 rdf:resource="http://purl.obolibrary.org/obo/GAZ_00280522"/>
        <obo:IAO_0000115>A bay.</obo:IAO_0000115>
        <oboInOwl:hasOBONamespace>GAZ</oboInOwl:hasOBONamespace>
        <oboInOwl:id>GAZ:00280466</oboInOwl:id>
        <rdfs:label>Hindisvik</rdfs:label>
    </owl:NamedIndividual>
    


    <!-- http://purl.obolibrary.org/obo/GAZ_00280467 -->

    <owl:NamedIndividual rdf:about="http://purl.obolibrary.org/obo/GAZ_00280467">
        <obo:RO_0001025 rdf:resource="http://purl.obolibrary.org/obo/GAZ_00020052"/>
        <obo:RO_0001025 rdf:resource="http://purl.obolibrary.org/obo/GAZ_00145765"/>
        <obo:RO_0001025 rdf:resource="http://purl.obolibrary.org/obo/GAZ_00280523"/>
        <obo:IAO_0000115>A bay.</obo:IAO_0000115>
        <oboInOwl:hasOBONamespace>GAZ</oboInOwl:hasOBONamespace>
        <oboInOwl:id>GAZ:00280467</oboInOwl:id>
        <rdfs:label>Hloduvik</rdfs:label>
    </owl:NamedIndividual>
    


    <!-- http://purl.obolibrary.org/obo/GAZ_00280468 -->

    <owl:NamedIndividual rdf:about="http://purl.obolibrary.org/obo/GAZ_00280468">
        <obo:RO_0001025 rdf:resource="http://purl.obolibrary.org/obo/GAZ_00001203"/>
        <obo:RO_0001025 rdf:resource="http://purl.obolibrary.org/obo/GAZ_00280522"/>
        <obo:IAO_0000115>A bay.</obo:IAO_0000115>
        <oboInOwl:hasOBONamespace>GAZ</oboInOwl:hasOBONamespace>
        <oboInOwl:id>GAZ:00280468</oboInOwl:id>
        <rdfs:label>Husavik i Vikum</rdfs:label>
    </owl:NamedIndividual>
    


    <!-- http://purl.obolibrary.org/obo/GAZ_00280469 -->

    <owl:NamedIndividual rdf:about="http://purl.obolibrary.org/obo/GAZ_00280469">
        <obo:RO_0001025 rdf:resource="http://purl.obolibrary.org/obo/GAZ_00145755"/>
        <obo:IAO_0000115>A bay.</obo:IAO_0000115>
        <oboInOwl:hasOBONamespace>GAZ</oboInOwl:hasOBONamespace>
        <oboInOwl:id>GAZ:00280469</oboInOwl:id>
        <rdfs:label>Kaldalon</rdfs:label>
    </owl:NamedIndividual>
    


    <!-- http://purl.obolibrary.org/obo/GAZ_00280470 -->

    <owl:NamedIndividual rdf:about="http://purl.obolibrary.org/obo/GAZ_00280470">
        <obo:RO_0001025 rdf:resource="http://purl.obolibrary.org/obo/GAZ_00001204"/>
        <obo:IAO_0000115>A lagoon.</obo:IAO_0000115>
        <oboInOwl:hasOBONamespace>GAZ</oboInOwl:hasOBONamespace>
        <oboInOwl:id>GAZ:00280470</oboInOwl:id>
        <rdfs:label>Lon</rdfs:label>
    </owl:NamedIndividual>
    


    <!-- http://purl.obolibrary.org/obo/GAZ_00280471 -->

    <owl:NamedIndividual rdf:about="http://purl.obolibrary.org/obo/GAZ_00280471">
        <obo:RO_0001025 rdf:resource="http://purl.obolibrary.org/obo/GAZ_00001208"/>
        <obo:RO_0001025 rdf:resource="http://purl.obolibrary.org/obo/GAZ_00280523"/>
        <obo:IAO_0000115>A bay.</obo:IAO_0000115>
        <oboInOwl:hasOBONamespace>GAZ</oboInOwl:hasOBONamespace>
        <oboInOwl:id>GAZ:00280471</oboInOwl:id>
        <rdfs:label>Straumsvik</rdfs:label>
    </owl:NamedIndividual>
    


    <!-- http://purl.obolibrary.org/obo/GAZ_00280472 -->

    <owl:NamedIndividual rdf:about="http://purl.obolibrary.org/obo/GAZ_00280472">
        <obo:RO_0001025 rdf:resource="http://purl.obolibrary.org/obo/GAZ_00280489"/>
        <obo:IAO_0000115>A bay.</obo:IAO_0000115>
        <oboInOwl:hasOBONamespace>GAZ</oboInOwl:hasOBONamespace>
        <oboInOwl:id>GAZ:00280472</oboInOwl:id>
        <rdfs:label>Trekyllisvik</rdfs:label>
    </owl:NamedIndividual>
    


    <!-- http://purl.obolibrary.org/obo/GAZ_00280473 -->

    <owl:NamedIndividual rdf:about="http://purl.obolibrary.org/obo/GAZ_00280473">
        <obo:RO_0001025 rdf:resource="http://purl.obolibrary.org/obo/GAZ_00020055"/>
        <obo:RO_0001025 rdf:resource="http://purl.obolibrary.org/obo/GAZ_00280522"/>
        <obo:IAO_0000115>A fjord.</obo:IAO_0000115>
        <oboInOwl:hasOBONamespace>GAZ</oboInOwl:hasOBONamespace>
        <oboInOwl:id>GAZ:00280473</oboInOwl:id>
        <rdfs:label>Bjarnarfjoerdur</rdfs:label>
    </owl:NamedIndividual>
    


    <!-- http://purl.obolibrary.org/obo/GAZ_00280474 -->

    <owl:NamedIndividual rdf:about="http://purl.obolibrary.org/obo/GAZ_00280474">
        <obo:RO_0001025 rdf:resource="http://purl.obolibrary.org/obo/GAZ_00020052"/>
        <obo:RO_0001025 rdf:resource="http://purl.obolibrary.org/obo/GAZ_00280523"/>
        <obo:IAO_0000115>A fjord.</obo:IAO_0000115>
        <oboInOwl:hasOBONamespace>GAZ</oboInOwl:hasOBONamespace>
        <oboInOwl:id>GAZ:00280474</oboInOwl:id>
        <rdfs:label>Dyrafjoerdur</rdfs:label>
    </owl:NamedIndividual>
    


    <!-- http://purl.obolibrary.org/obo/GAZ_00280475 -->

    <owl:NamedIndividual rdf:about="http://purl.obolibrary.org/obo/GAZ_00280475">
        <obo:RO_0001025 rdf:resource="http://purl.obolibrary.org/obo/GAZ_00020052"/>
        <obo:RO_0001025 rdf:resource="http://purl.obolibrary.org/obo/GAZ_00280523"/>
        <obo:IAO_0000115>A fjord.</obo:IAO_0000115>
        <oboInOwl:hasOBONamespace>GAZ</oboInOwl:hasOBONamespace>
        <oboInOwl:id>GAZ:00280475</oboInOwl:id>
        <rdfs:label>Furufjoerdur</rdfs:label>
    </owl:NamedIndividual>
    


    <!-- http://purl.obolibrary.org/obo/GAZ_00280476 -->

    <owl:NamedIndividual rdf:about="http://purl.obolibrary.org/obo/GAZ_00280476">
        <obo:RO_0001025 rdf:resource="http://purl.obolibrary.org/obo/GAZ_00145755"/>
        <obo:IAO_0000115>A bay.</obo:IAO_0000115>
        <oboInOwl:hasOBONamespace>GAZ</oboInOwl:hasOBONamespace>
        <oboInOwl:id>GAZ:00280476</oboInOwl:id>
        <rdfs:label>Bolungarvi</rdfs:label>
    </owl:NamedIndividual>
    


    <!-- http://purl.obolibrary.org/obo/GAZ_00280477 -->

    <owl:NamedIndividual rdf:about="http://purl.obolibrary.org/obo/GAZ_00280477">
        <obo:RO_0001025 rdf:resource="http://purl.obolibrary.org/obo/GAZ_00145755"/>
        <obo:IAO_0000115>A fjord.</obo:IAO_0000115>
        <oboInOwl:hasOBONamespace>GAZ</oboInOwl:hasOBONamespace>
        <oboInOwl:id>GAZ:00280477</oboInOwl:id>
        <rdfs:label>Skutulsfjoerdur</rdfs:label>
    </owl:NamedIndividual>
    


    <!-- http://purl.obolibrary.org/obo/GAZ_00280478 -->

    <owl:NamedIndividual rdf:about="http://purl.obolibrary.org/obo/GAZ_00280478">
        <obo:RO_0001025 rdf:resource="http://purl.obolibrary.org/obo/GAZ_00145755"/>
        <obo:IAO_0000115>A fjord.</obo:IAO_0000115>
        <oboInOwl:hasOBONamespace>GAZ</oboInOwl:hasOBONamespace>
        <oboInOwl:id>GAZ:00280478</oboInOwl:id>
        <rdfs:label>Hestfjoerdur</rdfs:label>
    </owl:NamedIndividual>
    


    <!-- http://purl.obolibrary.org/obo/GAZ_00280479 -->

    <owl:NamedIndividual rdf:about="http://purl.obolibrary.org/obo/GAZ_00280479">
        <obo:RO_0001025 rdf:resource="http://purl.obolibrary.org/obo/GAZ_00145755"/>
        <obo:IAO_0000115>A fjord.</obo:IAO_0000115>
        <oboInOwl:hasOBONamespace>GAZ</oboInOwl:hasOBONamespace>
        <oboInOwl:id>GAZ:00280479</oboInOwl:id>
        <rdfs:label>Skotufjoerdur</rdfs:label>
    </owl:NamedIndividual>
    


    <!-- http://purl.obolibrary.org/obo/GAZ_00280480 -->

    <owl:NamedIndividual rdf:about="http://purl.obolibrary.org/obo/GAZ_00280480">
        <obo:RO_0001025 rdf:resource="http://purl.obolibrary.org/obo/GAZ_00145755"/>
        <obo:IAO_0000115>A fjord.</obo:IAO_0000115>
        <oboInOwl:hasOBONamespace>GAZ</oboInOwl:hasOBONamespace>
        <oboInOwl:id>GAZ:00280480</oboInOwl:id>
        <rdfs:label>Vatnsfjoerdur</rdfs:label>
    </owl:NamedIndividual>
    


    <!-- http://purl.obolibrary.org/obo/GAZ_00280481 -->

    <owl:NamedIndividual rdf:about="http://purl.obolibrary.org/obo/GAZ_00280481">
        <obo:RO_0001025 rdf:resource="http://purl.obolibrary.org/obo/GAZ_00145755"/>
        <obo:IAO_0000115>A fjord.</obo:IAO_0000115>
        <oboInOwl:hasOBONamespace>GAZ</oboInOwl:hasOBONamespace>
        <oboInOwl:id>GAZ:00280481</oboInOwl:id>
        <rdfs:label>Isafjoerdur</rdfs:label>
    </owl:NamedIndividual>
    


    <!-- http://purl.obolibrary.org/obo/GAZ_00280482 -->

    <owl:NamedIndividual rdf:about="http://purl.obolibrary.org/obo/GAZ_00280482">
        <obo:RO_0001025 rdf:resource="http://purl.obolibrary.org/obo/GAZ_00020052"/>
        <obo:RO_0001025 rdf:resource="http://purl.obolibrary.org/obo/GAZ_00145755"/>
        <obo:IAO_0000115>A system of five fjords in Westfjords, Iceland, situated north of Isafjardardjup and south of the Hornstrandir peninsula.</obo:IAO_0000115>
        <oboInOwl:hasOBONamespace>GAZ</oboInOwl:hasOBONamespace>
        <oboInOwl:id>GAZ:00280482</oboInOwl:id>
        <rdfs:label>Jokulfirdir</rdfs:label>
    </owl:NamedIndividual>
    


    <!-- http://purl.obolibrary.org/obo/GAZ_00280483 -->

    <owl:NamedIndividual rdf:about="http://purl.obolibrary.org/obo/GAZ_00280483">
        <obo:RO_0001025 rdf:resource="http://purl.obolibrary.org/obo/GAZ_00280482"/>
        <obo:IAO_0000115>A fjord.</obo:IAO_0000115>
        <oboInOwl:hasOBONamespace>GAZ</oboInOwl:hasOBONamespace>
        <oboInOwl:id>GAZ:00280483</oboInOwl:id>
        <rdfs:label>Hesteyrarfjoerdur</rdfs:label>
    </owl:NamedIndividual>
    


    <!-- http://purl.obolibrary.org/obo/GAZ_00280484 -->

    <owl:NamedIndividual rdf:about="http://purl.obolibrary.org/obo/GAZ_00280484">
        <obo:RO_0001025 rdf:resource="http://purl.obolibrary.org/obo/GAZ_00280482"/>
        <obo:IAO_0000115>A fjord.</obo:IAO_0000115>
        <oboInOwl:hasOBONamespace>GAZ</oboInOwl:hasOBONamespace>
        <oboInOwl:id>GAZ:00280484</oboInOwl:id>
        <rdfs:label>Veidileysufjoerdur</rdfs:label>
    </owl:NamedIndividual>
    


    <!-- http://purl.obolibrary.org/obo/GAZ_00280485 -->

    <owl:NamedIndividual rdf:about="http://purl.obolibrary.org/obo/GAZ_00280485">
        <obo:RO_0001025 rdf:resource="http://purl.obolibrary.org/obo/GAZ_00280482"/>
        <obo:IAO_0000115>A fjord.</obo:IAO_0000115>
        <oboInOwl:hasOBONamespace>GAZ</oboInOwl:hasOBONamespace>
        <oboInOwl:id>GAZ:00280485</oboInOwl:id>
        <rdfs:label>Lonafjoerdur</rdfs:label>
    </owl:NamedIndividual>
    


    <!-- http://purl.obolibrary.org/obo/GAZ_00280486 -->

    <owl:NamedIndividual rdf:about="http://purl.obolibrary.org/obo/GAZ_00280486">
        <obo:RO_0001025 rdf:resource="http://purl.obolibrary.org/obo/GAZ_00280482"/>
        <obo:IAO_0000115>A fjord.</obo:IAO_0000115>
        <oboInOwl:hasOBONamespace>GAZ</oboInOwl:hasOBONamespace>
        <oboInOwl:id>GAZ:00280486</oboInOwl:id>
        <rdfs:label>Hrafnsfjoerdur</rdfs:label>
    </owl:NamedIndividual>
    


    <!-- http://purl.obolibrary.org/obo/GAZ_00280487 -->

    <owl:NamedIndividual rdf:about="http://purl.obolibrary.org/obo/GAZ_00280487">
        <obo:RO_0001025 rdf:resource="http://purl.obolibrary.org/obo/GAZ_00280482"/>
        <obo:IAO_0000115>A fjord.</obo:IAO_0000115>
        <oboInOwl:hasOBONamespace>GAZ</oboInOwl:hasOBONamespace>
        <oboInOwl:id>GAZ:00280487</oboInOwl:id>
        <rdfs:label>Leirufjoerdur</rdfs:label>
    </owl:NamedIndividual>
    


    <!-- http://purl.obolibrary.org/obo/GAZ_00280488 -->

    <owl:NamedIndividual rdf:about="http://purl.obolibrary.org/obo/GAZ_00280488">
        <obo:RO_0001025 rdf:resource="http://purl.obolibrary.org/obo/GAZ_00020055"/>
        <obo:RO_0001025 rdf:resource="http://purl.obolibrary.org/obo/GAZ_00280522"/>
        <obo:IAO_0000115>A bay.</obo:IAO_0000115>
        <oboInOwl:hasOBONamespace>GAZ</oboInOwl:hasOBONamespace>
        <oboInOwl:id>GAZ:00280488</oboInOwl:id>
        <rdfs:label>Kaldbaksvik</rdfs:label>
    </owl:NamedIndividual>
    


    <!-- http://purl.obolibrary.org/obo/GAZ_00280489 -->

    <owl:NamedIndividual rdf:about="http://purl.obolibrary.org/obo/GAZ_00280489">
        <obo:RO_0001025 rdf:resource="http://purl.obolibrary.org/obo/GAZ_00020055"/>
        <obo:RO_0001025 rdf:resource="http://purl.obolibrary.org/obo/GAZ_00280522"/>
        <obo:IAO_0000115>A fjord.</obo:IAO_0000115>
        <oboInOwl:hasOBONamespace>GAZ</oboInOwl:hasOBONamespace>
        <oboInOwl:id>GAZ:00280489</oboInOwl:id>
        <rdfs:label>Nordurfjoerdur</rdfs:label>
    </owl:NamedIndividual>
    


    <!-- http://purl.obolibrary.org/obo/GAZ_00280490 -->

    <owl:NamedIndividual rdf:about="http://purl.obolibrary.org/obo/GAZ_00280490">
        <obo:RO_0001025 rdf:resource="http://purl.obolibrary.org/obo/GAZ_00020049"/>
        <oboInOwl:hasOBONamespace>GAZ</oboInOwl:hasOBONamespace>
        <oboInOwl:id>GAZ:00280490</oboInOwl:id>
        <rdfs:label>Ofeigsfjardarfloi</rdfs:label>
    </owl:NamedIndividual>
    


    <!-- http://purl.obolibrary.org/obo/GAZ_00280491 -->

    <owl:NamedIndividual rdf:about="http://purl.obolibrary.org/obo/GAZ_00280491">
        <obo:RO_0001025 rdf:resource="http://purl.obolibrary.org/obo/GAZ_00280490"/>
        <obo:IAO_0000115>A bay.</obo:IAO_0000115>
        <oboInOwl:hasOBONamespace>GAZ</oboInOwl:hasOBONamespace>
        <oboInOwl:id>GAZ:00280491</oboInOwl:id>
        <rdfs:label>Eyvindarfjoerdur</rdfs:label>
    </owl:NamedIndividual>
    


    <!-- http://purl.obolibrary.org/obo/GAZ_00280492 -->

    <owl:NamedIndividual rdf:about="http://purl.obolibrary.org/obo/GAZ_00280492">
        <obo:RO_0001025 rdf:resource="http://purl.obolibrary.org/obo/GAZ_00280490"/>
        <obo:IAO_0000115>A fjord.</obo:IAO_0000115>
        <oboInOwl:hasOBONamespace>GAZ</oboInOwl:hasOBONamespace>
        <oboInOwl:id>GAZ:00280492</oboInOwl:id>
        <rdfs:label>Drangsvik</rdfs:label>
    </owl:NamedIndividual>
    


    <!-- http://purl.obolibrary.org/obo/GAZ_00280493 -->

    <owl:NamedIndividual rdf:about="http://purl.obolibrary.org/obo/GAZ_00280493">
        <obo:RO_0001025 rdf:resource="http://purl.obolibrary.org/obo/GAZ_00280490"/>
        <obo:IAO_0000115>A fjord.</obo:IAO_0000115>
        <oboInOwl:hasOBONamespace>GAZ</oboInOwl:hasOBONamespace>
        <oboInOwl:id>GAZ:00280493</oboInOwl:id>
        <rdfs:label>Ingolfsfjoerdur</rdfs:label>
    </owl:NamedIndividual>
    


    <!-- http://purl.obolibrary.org/obo/GAZ_00280494 -->

    <owl:NamedIndividual rdf:about="http://purl.obolibrary.org/obo/GAZ_00280494">
        <obo:RO_0001025 rdf:resource="http://purl.obolibrary.org/obo/GAZ_00280490"/>
        <obo:IAO_0000115>A fjord.</obo:IAO_0000115>
        <oboInOwl:hasOBONamespace>GAZ</oboInOwl:hasOBONamespace>
        <oboInOwl:id>GAZ:00280494</oboInOwl:id>
        <rdfs:label>Ofeigsfjoerdur</rdfs:label>
    </owl:NamedIndividual>
    


    <!-- http://purl.obolibrary.org/obo/GAZ_00280495 -->

    <owl:NamedIndividual rdf:about="http://purl.obolibrary.org/obo/GAZ_00280495">
        <obo:RO_0001025 rdf:resource="http://purl.obolibrary.org/obo/GAZ_00020058"/>
        <obo:RO_0001025 rdf:resource="http://purl.obolibrary.org/obo/GAZ_00280523"/>
        <obo:IAO_0000115>A fjord.</obo:IAO_0000115>
        <oboInOwl:hasOBONamespace>GAZ</oboInOwl:hasOBONamespace>
        <oboInOwl:id>GAZ:00280495</oboInOwl:id>
        <rdfs:label>Patreksfjoerdur</rdfs:label>
    </owl:NamedIndividual>
    


    <!-- http://purl.obolibrary.org/obo/GAZ_00280496 -->

    <owl:NamedIndividual rdf:about="http://purl.obolibrary.org/obo/GAZ_00280496">
        <obo:RO_0001025 rdf:resource="http://purl.obolibrary.org/obo/GAZ_00280495"/>
        <obo:IAO_0000115>A fjord.</obo:IAO_0000115>
        <oboInOwl:hasOBONamespace>GAZ</oboInOwl:hasOBONamespace>
        <oboInOwl:id>GAZ:00280496</oboInOwl:id>
        <rdfs:label>Talknafjoerdur</rdfs:label>
    </owl:NamedIndividual>
    


    <!-- http://purl.obolibrary.org/obo/GAZ_00280497 -->

    <owl:NamedIndividual rdf:about="http://purl.obolibrary.org/obo/GAZ_00280497">
        <obo:RO_0001025 rdf:resource="http://purl.obolibrary.org/obo/GAZ_00020055"/>
        <obo:RO_0001025 rdf:resource="http://purl.obolibrary.org/obo/GAZ_00280522"/>
        <obo:IAO_0000115>A fjord.</obo:IAO_0000115>
        <oboInOwl:hasOBONamespace>GAZ</oboInOwl:hasOBONamespace>
        <oboInOwl:id>GAZ:00280497</oboInOwl:id>
        <rdfs:label>Reykjarfjoerdur a Strondum</rdfs:label>
    </owl:NamedIndividual>
    


    <!-- http://purl.obolibrary.org/obo/GAZ_00280498 -->

    <owl:NamedIndividual rdf:about="http://purl.obolibrary.org/obo/GAZ_00280498">
        <obo:RO_0001025 rdf:resource="http://purl.obolibrary.org/obo/GAZ_00280497"/>
        <obo:IAO_0000115>A fjord.</obo:IAO_0000115>
        <oboInOwl:hasOBONamespace>GAZ</oboInOwl:hasOBONamespace>
        <oboInOwl:id>GAZ:00280498</oboInOwl:id>
        <rdfs:label>Veidileysa</rdfs:label>
    </owl:NamedIndividual>
    


    <!-- http://purl.obolibrary.org/obo/GAZ_00280499 -->

    <owl:NamedIndividual rdf:about="http://purl.obolibrary.org/obo/GAZ_00280499">
        <obo:RO_0001025 rdf:resource="http://purl.obolibrary.org/obo/GAZ_00020052"/>
        <obo:RO_0001025 rdf:resource="http://purl.obolibrary.org/obo/GAZ_00280523"/>
        <obo:IAO_0000115>A fjord.</obo:IAO_0000115>
        <oboInOwl:hasOBONamespace>GAZ</oboInOwl:hasOBONamespace>
        <oboInOwl:id>GAZ:00280499</oboInOwl:id>
        <rdfs:label>Reykjarfjoerdur nyrdri</rdfs:label>
    </owl:NamedIndividual>
    


    <!-- http://purl.obolibrary.org/obo/GAZ_00280500 -->

    <owl:NamedIndividual rdf:about="http://purl.obolibrary.org/obo/GAZ_00280500">
        <obo:RO_0001025 rdf:resource="http://purl.obolibrary.org/obo/GAZ_00020052"/>
        <obo:RO_0001025 rdf:resource="http://purl.obolibrary.org/obo/GAZ_00280523"/>
        <obo:IAO_0000115>A fjord.</obo:IAO_0000115>
        <oboInOwl:hasOBONamespace>GAZ</oboInOwl:hasOBONamespace>
        <oboInOwl:id>GAZ:00280500</oboInOwl:id>
        <rdfs:label>Sugandafjoerdur</rdfs:label>
    </owl:NamedIndividual>
    


    <!-- http://purl.obolibrary.org/obo/GAZ_00280501 -->

    <owl:NamedIndividual rdf:about="http://purl.obolibrary.org/obo/GAZ_00280501">
        <obo:RO_0001025 rdf:resource="http://purl.obolibrary.org/obo/GAZ_00020055"/>
        <obo:RO_0001025 rdf:resource="http://purl.obolibrary.org/obo/GAZ_00145764"/>
        <obo:RO_0001025 rdf:resource="http://purl.obolibrary.org/obo/GAZ_00280522"/>
        <obo:IAO_0000115>A fjord in Iceland.</obo:IAO_0000115>
        <oboInOwl:hasOBONamespace>GAZ</oboInOwl:hasOBONamespace>
        <oboInOwl:id>GAZ:00280501</oboInOwl:id>
        <rdfs:label>Steingrimsfjoerdur</rdfs:label>
    </owl:NamedIndividual>
    


    <!-- http://purl.obolibrary.org/obo/GAZ_00280502 -->

    <owl:NamedIndividual rdf:about="http://purl.obolibrary.org/obo/GAZ_00280502">
        <obo:RO_0001025 rdf:resource="http://purl.obolibrary.org/obo/GAZ_00145754"/>
        <obo:IAO_0000115>A fjord.</obo:IAO_0000115>
        <oboInOwl:hasOBONamespace>GAZ</oboInOwl:hasOBONamespace>
        <oboInOwl:id>GAZ:00280502</oboInOwl:id>
        <rdfs:label>Stakksfjoerdur</rdfs:label>
    </owl:NamedIndividual>
    


    <!-- http://purl.obolibrary.org/obo/GAZ_00280503 -->

    <owl:NamedIndividual rdf:about="http://purl.obolibrary.org/obo/GAZ_00280503">
        <obo:RO_0001025 rdf:resource="http://purl.obolibrary.org/obo/GAZ_00145754"/>
        <obo:IAO_0000115>A fjord.</obo:IAO_0000115>
        <oboInOwl:hasOBONamespace>GAZ</oboInOwl:hasOBONamespace>
        <oboInOwl:id>GAZ:00280503</oboInOwl:id>
        <rdfs:label>Hafnarfjoerdur</rdfs:label>
    </owl:NamedIndividual>
    


    <!-- http://purl.obolibrary.org/obo/GAZ_00280504 -->

    <owl:NamedIndividual rdf:about="http://purl.obolibrary.org/obo/GAZ_00280504">
        <obo:RO_0001025 rdf:resource="http://purl.obolibrary.org/obo/GAZ_00145754"/>
        <obo:IAO_0000115>A fjord.</obo:IAO_0000115>
        <oboInOwl:hasOBONamespace>GAZ</oboInOwl:hasOBONamespace>
        <oboInOwl:id>GAZ:00280504</oboInOwl:id>
        <rdfs:label>Haffjoerdur</rdfs:label>
    </owl:NamedIndividual>
    


    <!-- http://purl.obolibrary.org/obo/GAZ_00280505 -->

    <owl:NamedIndividual rdf:about="http://purl.obolibrary.org/obo/GAZ_00280505">
        <obo:RO_0001025 rdf:resource="http://purl.obolibrary.org/obo/GAZ_00145764"/>
        <obo:RO_0001025 rdf:resource="http://purl.obolibrary.org/obo/GAZ_00280522"/>
        <obo:IAO_0000115>A fjord.</obo:IAO_0000115>
        <oboInOwl:hasOBONamespace>GAZ</oboInOwl:hasOBONamespace>
        <oboInOwl:id>GAZ:00280505</oboInOwl:id>
        <rdfs:label>Tharalatursfjoerdur</rdfs:label>
    </owl:NamedIndividual>
    


    <!-- http://purl.obolibrary.org/obo/GAZ_00280506 -->

    <owl:NamedIndividual rdf:about="http://purl.obolibrary.org/obo/GAZ_00280506">
        <obo:RO_0001025 rdf:resource="http://purl.obolibrary.org/obo/GAZ_00145764"/>
        <obo:RO_0001025 rdf:resource="http://purl.obolibrary.org/obo/GAZ_00280522"/>
        <obo:IAO_0000115>A fjord.</obo:IAO_0000115>
        <oboInOwl:hasOBONamespace>GAZ</oboInOwl:hasOBONamespace>
        <oboInOwl:id>GAZ:00280506</oboInOwl:id>
        <rdfs:label>Bjarnarfjoerdur nyrori</rdfs:label>
    </owl:NamedIndividual>
    


    <!-- http://purl.obolibrary.org/obo/GAZ_00280507 -->

    <owl:NamedIndividual rdf:about="http://purl.obolibrary.org/obo/GAZ_00280507">
        <obo:RO_0001025 rdf:resource="http://purl.obolibrary.org/obo/GAZ_00145764"/>
        <obo:RO_0001025 rdf:resource="http://purl.obolibrary.org/obo/GAZ_00280523"/>
        <obo:IAO_0000115>A fjord.</obo:IAO_0000115>
        <oboInOwl:hasOBONamespace>GAZ</oboInOwl:hasOBONamespace>
        <oboInOwl:id>GAZ:00280507</oboInOwl:id>
        <rdfs:label>Veidileysufjoerdur</rdfs:label>
    </owl:NamedIndividual>
    


    <!-- http://purl.obolibrary.org/obo/GAZ_00280508 -->

    <owl:NamedIndividual rdf:about="http://purl.obolibrary.org/obo/GAZ_00280508">
        <obo:RO_0001025 rdf:resource="http://purl.obolibrary.org/obo/GAZ_00145764"/>
        <obo:RO_0001025 rdf:resource="http://purl.obolibrary.org/obo/GAZ_00280522"/>
        <obo:IAO_0000115>A fjord.</obo:IAO_0000115>
        <oboInOwl:hasOBONamespace>GAZ</oboInOwl:hasOBONamespace>
        <oboInOwl:id>GAZ:00280508</oboInOwl:id>
        <rdfs:label>Bitrufjoerdur</rdfs:label>
    </owl:NamedIndividual>
    


    <!-- http://purl.obolibrary.org/obo/GAZ_00280509 -->

    <owl:NamedIndividual rdf:about="http://purl.obolibrary.org/obo/GAZ_00280509">
        <obo:RO_0001025 rdf:resource="http://purl.obolibrary.org/obo/GAZ_00001207"/>
        <obo:RO_0001025 rdf:resource="http://purl.obolibrary.org/obo/GAZ_00280522"/>
        <obo:IAO_0000115>A fjord.</obo:IAO_0000115>
        <oboInOwl:hasOBONamespace>GAZ</oboInOwl:hasOBONamespace>
        <oboInOwl:id>GAZ:00280509</oboInOwl:id>
        <rdfs:label>Thorgeirsfjoerdur</rdfs:label>
    </owl:NamedIndividual>
    


    <!-- http://purl.obolibrary.org/obo/GAZ_00280510 -->

    <owl:NamedIndividual rdf:about="http://purl.obolibrary.org/obo/GAZ_00280510">
        <obo:RO_0001025 rdf:resource="http://purl.obolibrary.org/obo/GAZ_00001207"/>
        <obo:RO_0001025 rdf:resource="http://purl.obolibrary.org/obo/GAZ_00280522"/>
        <obo:IAO_0000115>A fjord.</obo:IAO_0000115>
        <oboInOwl:hasOBONamespace>GAZ</oboInOwl:hasOBONamespace>
        <oboInOwl:id>GAZ:00280510</oboInOwl:id>
        <rdfs:label>Hvalvatnsfjoerdur</rdfs:label>
    </owl:NamedIndividual>
    


    <!-- http://purl.obolibrary.org/obo/GAZ_00280511 -->

    <owl:NamedIndividual rdf:about="http://purl.obolibrary.org/obo/GAZ_00280511">
        <obo:RO_0001025 rdf:resource="http://purl.obolibrary.org/obo/GAZ_00145786"/>
        <obo:IAO_0000115>A fjord.</obo:IAO_0000115>
        <oboInOwl:hasOBONamespace>GAZ</oboInOwl:hasOBONamespace>
        <oboInOwl:id>GAZ:00280511</oboInOwl:id>
        <rdfs:label>Lonafjoerdur</rdfs:label>
    </owl:NamedIndividual>
    


    <!-- http://purl.obolibrary.org/obo/GAZ_00280512 -->

    <owl:NamedIndividual rdf:about="http://purl.obolibrary.org/obo/GAZ_00280512">
        <obo:RO_0001025 rdf:resource="http://purl.obolibrary.org/obo/GAZ_00145791"/>
        <obo:IAO_0000115>A fjord.</obo:IAO_0000115>
        <oboInOwl:hasOBONamespace>GAZ</oboInOwl:hasOBONamespace>
        <oboInOwl:id>GAZ:00280512</oboInOwl:id>
        <rdfs:label>Finnafjoerdur</rdfs:label>
    </owl:NamedIndividual>
    


    <!-- http://purl.obolibrary.org/obo/GAZ_00280513 -->

    <owl:NamedIndividual rdf:about="http://purl.obolibrary.org/obo/GAZ_00280513">
        <obo:RO_0001025 rdf:resource="http://purl.obolibrary.org/obo/GAZ_00145791"/>
        <obo:IAO_0000115>A fjord.</obo:IAO_0000115>
        <oboInOwl:hasOBONamespace>GAZ</oboInOwl:hasOBONamespace>
        <oboInOwl:id>GAZ:00280513</oboInOwl:id>
        <rdfs:label>Bakkafoerdur</rdfs:label>
    </owl:NamedIndividual>
    


    <!-- http://purl.obolibrary.org/obo/GAZ_00280514 -->

    <owl:NamedIndividual rdf:about="http://purl.obolibrary.org/obo/GAZ_00280514">
        <obo:RO_0001025 rdf:resource="http://purl.obolibrary.org/obo/GAZ_00020009"/>
        <obo:IAO_0000115>A fjord.</obo:IAO_0000115>
        <oboInOwl:hasOBONamespace>GAZ</oboInOwl:hasOBONamespace>
        <oboInOwl:id>GAZ:00280514</oboInOwl:id>
        <rdfs:label>Nypsfjoerdur</rdfs:label>
    </owl:NamedIndividual>
    


    <!-- http://purl.obolibrary.org/obo/GAZ_00280516 -->

    <owl:NamedIndividual rdf:about="http://purl.obolibrary.org/obo/GAZ_00280516">
        <obo:RO_0001025 rdf:resource="http://purl.obolibrary.org/obo/GAZ_00001203"/>
        <obo:RO_0001025 rdf:resource="http://purl.obolibrary.org/obo/GAZ_00280522"/>
        <obo:IAO_0000115>A bay.</obo:IAO_0000115>
        <oboInOwl:hasOBONamespace>GAZ</oboInOwl:hasOBONamespace>
        <oboInOwl:id>GAZ:00280516</oboInOwl:id>
        <rdfs:label>Nordfjardarfloi</rdfs:label>
    </owl:NamedIndividual>
    


    <!-- http://purl.obolibrary.org/obo/GAZ_00280517 -->

    <owl:NamedIndividual rdf:about="http://purl.obolibrary.org/obo/GAZ_00280517">
        <obo:RO_0001025 rdf:resource="http://purl.obolibrary.org/obo/GAZ_00280516"/>
        <obo:IAO_0000115>A fjord.</obo:IAO_0000115>
        <oboInOwl:hasOBONamespace>GAZ</oboInOwl:hasOBONamespace>
        <oboInOwl:id>GAZ:00280517</oboInOwl:id>
        <rdfs:label>Hellisfjoerdur</rdfs:label>
    </owl:NamedIndividual>
    


    <!-- http://purl.obolibrary.org/obo/GAZ_00280518 -->

    <owl:NamedIndividual rdf:about="http://purl.obolibrary.org/obo/GAZ_00280518">
        <obo:RO_0001025 rdf:resource="http://purl.obolibrary.org/obo/GAZ_00280516"/>
        <obo:IAO_0000115>A fjord.</obo:IAO_0000115>
        <oboInOwl:hasOBONamespace>GAZ</oboInOwl:hasOBONamespace>
        <oboInOwl:id>GAZ:00280518</oboInOwl:id>
        <rdfs:label>Vidfjoerdur</rdfs:label>
    </owl:NamedIndividual>
    


    <!-- http://purl.obolibrary.org/obo/GAZ_00280520 -->

    <owl:NamedIndividual rdf:about="http://purl.obolibrary.org/obo/GAZ_00280520">
        <obo:RO_0001025 rdf:resource="http://purl.obolibrary.org/obo/GAZ_00001203"/>
        <obo:IAO_0000115>A lagoon.</obo:IAO_0000115>
        <oboInOwl:hasOBONamespace>GAZ</oboInOwl:hasOBONamespace>
        <oboInOwl:id>GAZ:00280520</oboInOwl:id>
        <rdfs:label>Papafjoerdur</rdfs:label>
    </owl:NamedIndividual>
    


    <!-- http://purl.obolibrary.org/obo/GAZ_00280521 -->

    <owl:NamedIndividual rdf:about="http://purl.obolibrary.org/obo/GAZ_00280521">
        <obo:RO_0001025 rdf:resource="http://purl.obolibrary.org/obo/GAZ_00001203"/>
        <obo:IAO_0000115>A lagoon.</obo:IAO_0000115>
        <oboInOwl:hasOBONamespace>GAZ</oboInOwl:hasOBONamespace>
        <oboInOwl:id>GAZ:00280521</oboInOwl:id>
        <rdfs:label>Skardsfjoerdur</rdfs:label>
    </owl:NamedIndividual>
    


    <!-- http://purl.obolibrary.org/obo/GAZ_00280522 -->

    <owl:NamedIndividual rdf:about="http://purl.obolibrary.org/obo/GAZ_00280522">
        <obo:RO_0001025 rdf:resource="http://purl.obolibrary.org/obo/GAZ_00145753"/>
        <oboInOwl:hasOBONamespace>GAZ</oboInOwl:hasOBONamespace>
        <oboInOwl:id>GAZ:00280522</oboInOwl:id>
        <rdfs:label>Greenland Sea coastal waters of Iceland</rdfs:label>
    </owl:NamedIndividual>
    


    <!-- http://purl.obolibrary.org/obo/GAZ_00280523 -->

    <owl:NamedIndividual rdf:about="http://purl.obolibrary.org/obo/GAZ_00280523">
        <obo:RO_0001025 rdf:resource="http://purl.obolibrary.org/obo/GAZ_00145753"/>
        <oboInOwl:hasOBONamespace>GAZ</oboInOwl:hasOBONamespace>
        <oboInOwl:id>GAZ:00280523</oboInOwl:id>
        <rdfs:label>North Atlantic Ocean coastal waters of Iceland</rdfs:label>
    </owl:NamedIndividual>
    


    <!-- http://purl.obolibrary.org/obo/GAZ_00280527 -->

    <owl:NamedIndividual rdf:about="http://purl.obolibrary.org/obo/GAZ_00280527">
        <obo:RO_0001025 rdf:resource="http://purl.obolibrary.org/obo/GAZ_00001204"/>
        <obo:IAO_0000115>A sandur in S Iceland.</obo:IAO_0000115>
        <oboInOwl:hasOBONamespace>GAZ</oboInOwl:hasOBONamespace>
        <oboInOwl:id>GAZ:00280527</oboInOwl:id>
        <rdfs:label>Myrdalssandur</rdfs:label>
    </owl:NamedIndividual>
    


    <!-- http://purl.obolibrary.org/obo/GAZ_00280528 -->

    <owl:NamedIndividual rdf:about="http://purl.obolibrary.org/obo/GAZ_00280528">
        <obo:RO_0001025 rdf:resource="http://purl.obolibrary.org/obo/GAZ_00001204"/>
        <obo:IAO_0000115>A river. Rises in the Myrdalsjokull and discharges to the Atlantic Ocean across the Myrdalssandur.</obo:IAO_0000115>
        <oboInOwl:hasOBONamespace>GAZ</oboInOwl:hasOBONamespace>
        <oboInOwl:id>GAZ:00280528</oboInOwl:id>
        <rdfs:label>Kudafljot</rdfs:label>
    </owl:NamedIndividual>
    


    <!-- http://purl.obolibrary.org/obo/GAZ_00280530 -->

    <owl:NamedIndividual rdf:about="http://purl.obolibrary.org/obo/GAZ_00280530">
        <obo:RO_0001025 rdf:resource="http://purl.obolibrary.org/obo/GAZ_00001204"/>
        <obo:IAO_0000115>A river. Rises in the Myrdalsjokull and discharges to the Atlantic Ocean across the Myrdalssandur.</obo:IAO_0000115>
        <oboInOwl:hasOBONamespace>GAZ</oboInOwl:hasOBONamespace>
        <oboInOwl:id>GAZ:00280530</oboInOwl:id>
        <rdfs:label>Mulakvisl</rdfs:label>
    </owl:NamedIndividual>
    


    <!-- http://purl.obolibrary.org/obo/GAZ_00280531 -->

    <owl:NamedIndividual rdf:about="http://purl.obolibrary.org/obo/GAZ_00280531">
        <obo:RO_0001025 rdf:resource="http://purl.obolibrary.org/obo/GAZ_00001204"/>
        <obo:IAO_0000115>A river. Rises in the Myrkvavatn between Sulur and Burfell and discharges to Thingvallavatn.</obo:IAO_0000115>
        <oboInOwl:hasOBONamespace>GAZ</oboInOwl:hasOBONamespace>
        <oboInOwl:id>GAZ:00280531</oboInOwl:id>
        <rdfs:label>Oxara</rdfs:label>
    </owl:NamedIndividual>
    


    <!-- http://purl.obolibrary.org/obo/GAZ_00280532 -->

    <owl:NamedIndividual rdf:about="http://purl.obolibrary.org/obo/GAZ_00280532">
        <obo:RO_0001025 rdf:resource="http://purl.obolibrary.org/obo/GAZ_00001204"/>
        <oboInOwl:hasOBONamespace>GAZ</oboInOwl:hasOBONamespace>
        <oboInOwl:id>GAZ:00280532</oboInOwl:id>
        <rdfs:label>Eystri-Ranga</rdfs:label>
    </owl:NamedIndividual>
    


    <!-- http://purl.obolibrary.org/obo/GAZ_00280533 -->

    <owl:NamedIndividual rdf:about="http://purl.obolibrary.org/obo/GAZ_00280533">
        <obo:RO_0001025 rdf:resource="http://purl.obolibrary.org/obo/GAZ_00001204"/>
        <obo:IAO_0000115>A river. It has its source on the glacier Skeidararjokull.</obo:IAO_0000115>
        <oboInOwl:hasOBONamespace>GAZ</oboInOwl:hasOBONamespace>
        <oboInOwl:id>GAZ:00280533</oboInOwl:id>
        <rdfs:label>Skeidara</rdfs:label>
    </owl:NamedIndividual>
    


    <!-- http://purl.obolibrary.org/obo/GAZ_00280536 -->

    <owl:NamedIndividual rdf:about="http://purl.obolibrary.org/obo/GAZ_00280536">
        <obo:RO_0001025 rdf:resource="http://purl.obolibrary.org/obo/GAZ_00001204"/>
        <obo:IAO_0000115>A river.</obo:IAO_0000115>
        <oboInOwl:hasOBONamespace>GAZ</oboInOwl:hasOBONamespace>
        <oboInOwl:id>GAZ:00280536</oboInOwl:id>
        <rdfs:label>Ytri-Ranga</rdfs:label>
    </owl:NamedIndividual>
    


    <!-- http://purl.obolibrary.org/obo/GAZ_00280537 -->

    <owl:NamedIndividual rdf:about="http://purl.obolibrary.org/obo/GAZ_00280537">
        <obo:RO_0001025 rdf:resource="http://purl.obolibrary.org/obo/GAZ_00001204"/>
        <obo:IAO_0000115>A river.</obo:IAO_0000115>
        <oboInOwl:hasOBONamespace>GAZ</oboInOwl:hasOBONamespace>
        <oboInOwl:id>GAZ:00280537</oboInOwl:id>
        <rdfs:label>Thvera</rdfs:label>
    </owl:NamedIndividual>
    


    <!-- http://purl.obolibrary.org/obo/GAZ_00280544 -->

    <owl:NamedIndividual rdf:about="http://purl.obolibrary.org/obo/GAZ_00280544">
        <rdf:type rdf:resource="http://purl.obolibrary.org/obo/ENVO_00000475"/>
        <obo:RO_0001025 rdf:resource="http://purl.obolibrary.org/obo/GAZ_00053316"/>
        <obo:IAO_0000115>A glacier. An arm of Vatnajokull.</obo:IAO_0000115>
        <oboInOwl:hasOBONamespace>GAZ</oboInOwl:hasOBONamespace>
        <oboInOwl:id>GAZ:00280544</oboInOwl:id>
        <rdfs:label>Skeidararjokull</rdfs:label>
    </owl:NamedIndividual>
    


    <!-- http://purl.obolibrary.org/obo/GAZ_00280545 -->

    <owl:NamedIndividual rdf:about="http://purl.obolibrary.org/obo/GAZ_00280545">
        <rdf:type rdf:resource="http://purl.obolibrary.org/obo/ENVO_00000104"/>
        <obo:RO_0001025 rdf:resource="http://purl.obolibrary.org/obo/GAZ_00053316"/>
        <obo:RO_0001025 rdf:resource="http://purl.obolibrary.org/obo/GAZ_00062056"/>
        <obo:IAO_0000115>A glacier. A spur of the Vatnajokull.</obo:IAO_0000115>
        <oboInOwl:hasOBONamespace>GAZ</oboInOwl:hasOBONamespace>
        <oboInOwl:id>GAZ:00280545</oboInOwl:id>
        <rdfs:label>Skaftafellsjokull</rdfs:label>
    </owl:NamedIndividual>
    


    <!-- http://purl.obolibrary.org/obo/GAZ_00280546 -->

    <owl:NamedIndividual rdf:about="http://purl.obolibrary.org/obo/GAZ_00280546">
        <obo:RO_0001025 rdf:resource="http://purl.obolibrary.org/obo/GAZ_00001206"/>
        <obo:IAO_0000115>A river. Rises in the Hallmundarhraun and discharges to the Borgarfjoerdur.</obo:IAO_0000115>
        <oboInOwl:hasOBONamespace>GAZ</oboInOwl:hasOBONamespace>
        <oboInOwl:id>GAZ:00280546</oboInOwl:id>
        <rdfs:label>Hvita</rdfs:label>
    </owl:NamedIndividual>
    


    <!-- http://purl.obolibrary.org/obo/GAZ_00280549 -->

    <owl:NamedIndividual rdf:about="http://purl.obolibrary.org/obo/GAZ_00280549">
        <obo:RO_0001025 rdf:resource="http://purl.obolibrary.org/obo/GAZ_00001206"/>
        <obo:IAO_0000115>A lava field.</obo:IAO_0000115>
        <oboInOwl:hasOBONamespace>GAZ</oboInOwl:hasOBONamespace>
        <oboInOwl:id>GAZ:00280549</oboInOwl:id>
        <rdfs:label>Hallmundarhraun</rdfs:label>
    </owl:NamedIndividual>
    


    <!-- http://purl.obolibrary.org/obo/GAZ_00280550 -->

    <owl:NamedIndividual rdf:about="http://purl.obolibrary.org/obo/GAZ_00280550">
        <obo:RO_0001025 rdf:resource="http://purl.obolibrary.org/obo/GAZ_00145764"/>
        <obo:IAO_0000115>A river.</obo:IAO_0000115>
        <oboInOwl:hasOBONamespace>GAZ</oboInOwl:hasOBONamespace>
        <oboInOwl:id>GAZ:00280550</oboInOwl:id>
        <rdfs:label>Dynjandisa</rdfs:label>
    </owl:NamedIndividual>
    


    <!-- http://purl.obolibrary.org/obo/GAZ_00280562 -->

    <owl:NamedIndividual rdf:about="http://purl.obolibrary.org/obo/GAZ_00280562">
        <obo:RO_0001025 rdf:resource="http://purl.obolibrary.org/obo/GAZ_00001207"/>
        <obo:IAO_0000115>A lava field.</obo:IAO_0000115>
        <oboInOwl:hasOBONamespace>GAZ</oboInOwl:hasOBONamespace>
        <oboInOwl:id>GAZ:00280562</oboInOwl:id>
        <rdfs:label>Odadahraun</rdfs:label>
    </owl:NamedIndividual>
    


    <!-- http://purl.obolibrary.org/obo/GAZ_00280564 -->

    <owl:NamedIndividual rdf:about="http://purl.obolibrary.org/obo/GAZ_00280564">
        <obo:RO_0001025 rdf:resource="http://purl.obolibrary.org/obo/GAZ_00280137"/>
        <obo:IAO_0000115>A waterfall in the river Jokulsa a Fjollum in the north of Iceland which drops over some waterfalls about 30 km before flowing into Oxarfjoerdur, a bay of the Arctic Sea.</obo:IAO_0000115>
        <oboInOwl:hasOBONamespace>GAZ</oboInOwl:hasOBONamespace>
        <oboInOwl:id>GAZ:00280564</oboInOwl:id>
        <rdfs:label>Selfoss</rdfs:label>
    </owl:NamedIndividual>
    


    <!-- http://purl.obolibrary.org/obo/GAZ_00280565 -->

    <owl:NamedIndividual rdf:about="http://purl.obolibrary.org/obo/GAZ_00280565">
        <obo:RO_0001025 rdf:resource="http://purl.obolibrary.org/obo/GAZ_00089838"/>
        <obo:RO_0001025 rdf:resource="http://purl.obolibrary.org/obo/GAZ_00280137"/>
        <obo:IAO_0000115>A waterfall in Jokulsargljufur National Park of Northeast Iceland. It is situated on the Jokulsa a Fjollum.</obo:IAO_0000115>
        <oboInOwl:hasOBONamespace>GAZ</oboInOwl:hasOBONamespace>
        <oboInOwl:id>GAZ:00280565</oboInOwl:id>
        <rdfs:label>Dettifoss</rdfs:label>
    </owl:NamedIndividual>
    


    <!-- http://purl.obolibrary.org/obo/GAZ_00432284 -->

    <owl:NamedIndividual rdf:about="http://purl.obolibrary.org/obo/GAZ_00432284">
        <obo:IAO_0000115>An airport.</obo:IAO_0000115>
        <oboInOwl:hasOBONamespace>GAZ</oboInOwl:hasOBONamespace>
        <oboInOwl:id>GAZ:00432284</oboInOwl:id>
        <rdfs:label>Keflavik International Airport</rdfs:label>
    </owl:NamedIndividual>
    


    <!-- http://purl.obolibrary.org/obo/GAZ_02000603 -->

    <owl:NamedIndividual rdf:about="http://purl.obolibrary.org/obo/GAZ_02000603">
        <rdf:type rdf:resource="http://purl.obolibrary.org/obo/ENVO_00000856"/>
        <obo:RO_0001025 rdf:resource="http://purl.obolibrary.org/obo/GAZ_00001208"/>
        <obo:IAO_0000115>A municipality.</obo:IAO_0000115>
        <oboInOwl:hasOBONamespace>GAZ</oboInOwl:hasOBONamespace>
        <oboInOwl:id>GAZ:02000603</oboInOwl:id>
        <rdfs:label>Municipality of Reykjavik</rdfs:label>
    </owl:NamedIndividual>
    


    <!-- http://purl.obolibrary.org/obo/GAZ_02000604 -->

    <owl:NamedIndividual rdf:about="http://purl.obolibrary.org/obo/GAZ_02000604">
        <rdf:type rdf:resource="http://purl.obolibrary.org/obo/ENVO_00000856"/>
        <obo:RO_0001025 rdf:resource="http://purl.obolibrary.org/obo/GAZ_00001204"/>
        <obo:IAO_0000115>A municipality.</obo:IAO_0000115>
        <oboInOwl:hasOBONamespace>GAZ</oboInOwl:hasOBONamespace>
        <oboInOwl:id>GAZ:02000604</oboInOwl:id>
        <rdfs:label>Municipality of Vestmannaeyjabaer</rdfs:label>
    </owl:NamedIndividual>
    


    <!-- http://purl.obolibrary.org/obo/GAZ_02000605 -->

    <owl:NamedIndividual rdf:about="http://purl.obolibrary.org/obo/GAZ_02000605">
        <rdf:type rdf:resource="http://purl.obolibrary.org/obo/ENVO_00000856"/>
        <obo:RO_0001025 rdf:resource="http://purl.obolibrary.org/obo/GAZ_00001204"/>
        <obo:IAO_0000115>A municipality.</obo:IAO_0000115>
        <oboInOwl:hasOBONamespace>GAZ</oboInOwl:hasOBONamespace>
        <oboInOwl:id>GAZ:02000605</oboInOwl:id>
        <rdfs:label>Sveitarfelagid Arborg</rdfs:label>
    </owl:NamedIndividual>
    


    <!-- 
    ///////////////////////////////////////////////////////////////////////////////////////
    //
    // Annotations
    //
    ///////////////////////////////////////////////////////////////////////////////////////
     -->

    <rdf:Description rdf:about="http://purl.obolibrary.org/obo/GAZ_00001200">
        <rdfs:label>Region (Iceland)</rdfs:label>
        <oboInOwl:id>GAZ:00001200</oboInOwl:id>
        <oboInOwl:hasOBONamespace>GAZ</oboInOwl:hasOBONamespace>
    </rdf:Description>
    <rdf:Description rdf:about="http://purl.obolibrary.org/obo/GAZ_00001201">
        <oboInOwl:id>GAZ:00001201</oboInOwl:id>
        <rdfs:label>Southern Penninsula Region</rdfs:label>
        <obo:IAO_0000115>A region in southwest Iceland.</obo:IAO_0000115>
        <oboInOwl:hasOBONamespace>GAZ</oboInOwl:hasOBONamespace>
    </rdf:Description>
    <rdf:Description rdf:about="http://purl.obolibrary.org/obo/GAZ_00001202">
        <rdfs:label>Northland West Region</rdfs:label>
        <obo:IAO_0000115>A region in the N of Iceland.</obo:IAO_0000115>
        <oboInOwl:id>GAZ:00001202</oboInOwl:id>
        <oboInOwl:hasOBONamespace>GAZ</oboInOwl:hasOBONamespace>
    </rdf:Description>
    <rdf:Description rdf:about="http://purl.obolibrary.org/obo/GAZ_00001203">
        <rdfs:label>Eastland Region</rdfs:label>
        <oboInOwl:id>GAZ:00001203</oboInOwl:id>
        <oboInOwl:hasOBONamespace>GAZ</oboInOwl:hasOBONamespace>
        <obo:IAO_0000115>A region in the E of Iceland.</obo:IAO_0000115>
    </rdf:Description>
    <rdf:Description rdf:about="http://purl.obolibrary.org/obo/GAZ_00001204">
        <rdfs:label>Southland Region</rdfs:label>
        <oboInOwl:id>GAZ:00001204</oboInOwl:id>
        <oboInOwl:hasOBONamespace>GAZ</oboInOwl:hasOBONamespace>
        <obo:IAO_0000115>A region in the S of Iceland.</obo:IAO_0000115>
    </rdf:Description>
    <rdf:Description rdf:about="http://purl.obolibrary.org/obo/GAZ_00001205">
        <obo:IAO_0000115>A region in the NW of Iceland on the Wesfjords Peninsula.</obo:IAO_0000115>
        <oboInOwl:id>GAZ:00001205</oboInOwl:id>
        <rdfs:label>Western Fjords Region</rdfs:label>
        <oboInOwl:hasOBONamespace>GAZ</oboInOwl:hasOBONamespace>
    </rdf:Description>
    <rdf:Description rdf:about="http://purl.obolibrary.org/obo/GAZ_00001206">
        <rdfs:label>Westland Region</rdfs:label>
        <obo:IAO_0000115>A region in the W of Iceland.</obo:IAO_0000115>
        <oboInOwl:hasOBONamespace>GAZ</oboInOwl:hasOBONamespace>
        <oboInOwl:id>GAZ:00001206</oboInOwl:id>
    </rdf:Description>
    <rdf:Description rdf:about="http://purl.obolibrary.org/obo/GAZ_00001207">
        <obo:IAO_0000115>A region in the N of Iceland.</obo:IAO_0000115>
        <rdfs:label>Northland East Region</rdfs:label>
        <oboInOwl:id>GAZ:00001207</oboInOwl:id>
        <oboInOwl:hasOBONamespace>GAZ</oboInOwl:hasOBONamespace>
    </rdf:Description>
    <rdf:Description rdf:about="http://purl.obolibrary.org/obo/GAZ_00001208">
        <rdfs:label>Capital Region</rdfs:label>
        <oboInOwl:hasOBONamespace>GAZ</oboInOwl:hasOBONamespace>
        <oboInOwl:id>GAZ:00001208</oboInOwl:id>
        <obo:IAO_0000115>The metropolitan area of the Icelandic capital Reykjavik.</obo:IAO_0000115>
    </rdf:Description>
    <rdf:Description rdf:about="http://purl.obolibrary.org/obo/GAZ_00007698">
        <oboInOwl:id>GAZ:00007698</oboInOwl:id>
        <rdfs:label>populated place, Iceland</rdfs:label>
        <oboInOwl:hasOBONamespace>GAZ</oboInOwl:hasOBONamespace>
    </rdf:Description>
    <rdf:Description rdf:about="http://purl.obolibrary.org/obo/GAZ_00007699">
        <oboInOwl:id>GAZ:00007699</oboInOwl:id>
        <rdfs:label>Selfoss</rdfs:label>
        <oboInOwl:hasOBONamespace>GAZ</oboInOwl:hasOBONamespace>
    </rdf:Description>
    <rdf:Description rdf:about="http://purl.obolibrary.org/obo/GAZ_00008737">
        <rdfs:label>City of Reykjavik</rdfs:label>
        <obo:IAO_0000115>The capital and largest city of Iceland.</obo:IAO_0000115>
        <oboInOwl:id>GAZ:00008737</oboInOwl:id>
        <oboInOwl:hasOBONamespace>GAZ</oboInOwl:hasOBONamespace>
    </rdf:Description>
    <rdf:Description rdf:about="http://purl.obolibrary.org/obo/GAZ_00280387">
        <rdfs:label>Gjabakkahraun</rdfs:label>
        <obo:IAO_0000115>A lava field.</obo:IAO_0000115>
        <oboInOwl:hasOBONamespace>GAZ</oboInOwl:hasOBONamespace>
        <oboInOwl:id>GAZ:00280387</oboInOwl:id>
    </rdf:Description>
</rdf:RDF>



<!-- Generated by the OWL API (version 4.5.6) https://github.com/owlcs/owlapi -->

