<?xml version="1.0"?>
<rdf:RDF xmlns="http://purl.obolibrary.org/obo/gaz/subsets/countries/Iraq.owl#"
     xml:base="http://purl.obolibrary.org/obo/gaz/subsets/countries/Iraq.owl"
     xmlns:obo="http://purl.obolibrary.org/obo/"
     xmlns:owl="http://www.w3.org/2002/07/owl#"
     xmlns:rdf="http://www.w3.org/1999/02/22-rdf-syntax-ns#"
     xmlns:xml="http://www.w3.org/XML/1998/namespace"
     xmlns:xsd="http://www.w3.org/2001/XMLSchema#"
     xmlns:rdfs="http://www.w3.org/2000/01/rdf-schema#"
     xmlns:oboInOwl="http://www.geneontology.org/formats/oboInOwl#">
    <owl:Ontology rdf:about="http://purl.obolibrary.org/obo/gaz/subsets/countries/Iraq.owl">
        <owl:imports rdf:resource="http://purl.obolibrary.org/obo/gaz/imports/envo_import.owl"/>
        <owl:imports rdf:resource="http://purl.obolibrary.org/obo/gaz/imports/ro_import.owl"/>
    </owl:Ontology>
    


    <!-- 
    ///////////////////////////////////////////////////////////////////////////////////////
    //
    // Annotation properties
    //
    ///////////////////////////////////////////////////////////////////////////////////////
     -->

    


    <!-- http://purl.obolibrary.org/obo/IAO_0000115 -->

    <owl:AnnotationProperty rdf:about="http://purl.obolibrary.org/obo/IAO_0000115"/>
    


    <!-- http://www.geneontology.org/formats/oboInOwl#hasOBONamespace -->

    <owl:AnnotationProperty rdf:about="http://www.geneontology.org/formats/oboInOwl#hasOBONamespace"/>
    


    <!-- http://www.geneontology.org/formats/oboInOwl#id -->

    <owl:AnnotationProperty rdf:about="http://www.geneontology.org/formats/oboInOwl#id"/>
    


    <!-- 
    ///////////////////////////////////////////////////////////////////////////////////////
    //
    // Object Properties
    //
    ///////////////////////////////////////////////////////////////////////////////////////
     -->

    


    <!-- http://purl.obolibrary.org/obo/RO_0001025 -->

    <owl:ObjectProperty rdf:about="http://purl.obolibrary.org/obo/RO_0001025"/>
    


    <!-- 
    ///////////////////////////////////////////////////////////////////////////////////////
    //
    // Classes
    //
    ///////////////////////////////////////////////////////////////////////////////////////
     -->

    


    <!-- http://purl.obolibrary.org/obo/ENVO_00000004 -->

    <owl:Class rdf:about="http://purl.obolibrary.org/obo/ENVO_00000004"/>
    


    <!-- http://purl.obolibrary.org/obo/ENVO_00000009 -->

    <owl:Class rdf:about="http://purl.obolibrary.org/obo/ENVO_00000009"/>
    


    <!-- http://purl.obolibrary.org/obo/ENVO_00000074 -->

    <owl:Class rdf:about="http://purl.obolibrary.org/obo/ENVO_00000074"/>
    


    <!-- http://purl.obolibrary.org/obo/ENVO_00000167 -->

    <owl:Class rdf:about="http://purl.obolibrary.org/obo/ENVO_00000167"/>
    


    <!-- http://purl.obolibrary.org/obo/ENVO_00000475 -->

    <owl:Class rdf:about="http://purl.obolibrary.org/obo/ENVO_00000475"/>
    


    <!-- http://purl.obolibrary.org/obo/ENVO_00000856 -->

    <owl:Class rdf:about="http://purl.obolibrary.org/obo/ENVO_00000856"/>
    


    <!-- http://purl.obolibrary.org/obo/GAZ_00004491 -->

    <owl:Class rdf:about="http://purl.obolibrary.org/obo/GAZ_00004491"/>
    


    <!-- http://purl.obolibrary.org/obo/GAZ_00004492 -->

    <owl:Class rdf:about="http://purl.obolibrary.org/obo/GAZ_00004492">
        <rdfs:subClassOf rdf:resource="http://purl.obolibrary.org/obo/GAZ_00004491"/>
    </owl:Class>
    


    <!-- http://purl.obolibrary.org/obo/GAZ_00004493 -->

    <owl:Class rdf:about="http://purl.obolibrary.org/obo/GAZ_00004493">
        <rdfs:subClassOf rdf:resource="http://purl.obolibrary.org/obo/GAZ_00004495"/>
    </owl:Class>
    


    <!-- http://purl.obolibrary.org/obo/GAZ_00004495 -->

    <owl:Class rdf:about="http://purl.obolibrary.org/obo/GAZ_00004495"/>
    


    <!-- http://purl.obolibrary.org/obo/GAZ_00009519 -->

    <owl:Class rdf:about="http://purl.obolibrary.org/obo/GAZ_00009519"/>
    


    <!-- http://purl.obolibrary.org/obo/GAZ_00010359 -->

    <owl:Class rdf:about="http://purl.obolibrary.org/obo/GAZ_00010359">
        <rdfs:subClassOf rdf:resource="http://purl.obolibrary.org/obo/GAZ_00004491"/>
    </owl:Class>
    


    <!-- http://purl.obolibrary.org/obo/GAZ_00010360 -->

    <owl:Class rdf:about="http://purl.obolibrary.org/obo/GAZ_00010360">
        <rdfs:subClassOf rdf:resource="http://purl.obolibrary.org/obo/GAZ_00004495"/>
    </owl:Class>
    


    <!-- http://purl.obolibrary.org/obo/GAZ_00030835 -->

    <owl:Class rdf:about="http://purl.obolibrary.org/obo/GAZ_00030835">
        <rdfs:subClassOf rdf:resource="http://purl.obolibrary.org/obo/GAZ_00004491"/>
    </owl:Class>
    


    <!-- http://purl.obolibrary.org/obo/GAZ_00052482 -->

    <owl:Class rdf:about="http://purl.obolibrary.org/obo/GAZ_00052482">
        <rdfs:subClassOf rdf:resource="http://purl.obolibrary.org/obo/GAZ_00004495"/>
    </owl:Class>
    


    <!-- http://purl.obolibrary.org/obo/GAZ_00052483 -->

    <owl:Class rdf:about="http://purl.obolibrary.org/obo/GAZ_00052483">
        <rdfs:subClassOf rdf:resource="http://purl.obolibrary.org/obo/GAZ_00004495"/>
    </owl:Class>
    


    <!-- http://purl.obolibrary.org/obo/GAZ_00052484 -->

    <owl:Class rdf:about="http://purl.obolibrary.org/obo/GAZ_00052484">
        <rdfs:subClassOf rdf:resource="http://purl.obolibrary.org/obo/GAZ_00004495"/>
    </owl:Class>
    


    <!-- http://purl.obolibrary.org/obo/GAZ_00052486 -->

    <owl:Class rdf:about="http://purl.obolibrary.org/obo/GAZ_00052486">
        <rdfs:subClassOf rdf:resource="http://purl.obolibrary.org/obo/GAZ_00004495"/>
    </owl:Class>
    


    <!-- http://purl.obolibrary.org/obo/GAZ_00052487 -->

    <owl:Class rdf:about="http://purl.obolibrary.org/obo/GAZ_00052487">
        <rdfs:subClassOf rdf:resource="http://purl.obolibrary.org/obo/GAZ_00004495"/>
    </owl:Class>
    


    <!-- http://purl.obolibrary.org/obo/GAZ_00052488 -->

    <owl:Class rdf:about="http://purl.obolibrary.org/obo/GAZ_00052488">
        <rdfs:subClassOf rdf:resource="http://purl.obolibrary.org/obo/GAZ_00004495"/>
    </owl:Class>
    


    <!-- http://purl.obolibrary.org/obo/GAZ_00053729 -->

    <owl:Class rdf:about="http://purl.obolibrary.org/obo/GAZ_00053729"/>
    


    <!-- http://purl.obolibrary.org/obo/GAZ_00251011 -->

    <owl:Class rdf:about="http://purl.obolibrary.org/obo/GAZ_00251011">
        <rdfs:subClassOf rdf:resource="http://purl.obolibrary.org/obo/GAZ_02000616"/>
        <obo:IAO_0000115>A saline lake. Located on the plains to the east of the Tigris River, 30 kin northeast of Samarra, Salah Al Din Governorate.</obo:IAO_0000115>
        <oboInOwl:hasOBONamespace>GAZ</oboInOwl:hasOBONamespace>
        <oboInOwl:id>GAZ:00251011</oboInOwl:id>
        <rdfs:label>Shari Lake</rdfs:label>
    </owl:Class>
    


    <!-- http://purl.obolibrary.org/obo/GAZ_02000358 -->

    <owl:Class rdf:about="http://purl.obolibrary.org/obo/GAZ_02000358">
        <rdfs:subClassOf rdf:resource="http://purl.obolibrary.org/obo/GAZ_00009519"/>
    </owl:Class>
    


    <!-- http://purl.obolibrary.org/obo/GAZ_02000359 -->

    <owl:Class rdf:about="http://purl.obolibrary.org/obo/GAZ_02000359">
        <rdfs:subClassOf rdf:resource="http://purl.obolibrary.org/obo/GAZ_00009519"/>
    </owl:Class>
    


    <!-- http://purl.obolibrary.org/obo/GAZ_02000360 -->

    <owl:Class rdf:about="http://purl.obolibrary.org/obo/GAZ_02000360">
        <rdfs:subClassOf rdf:resource="http://purl.obolibrary.org/obo/GAZ_00009519"/>
    </owl:Class>
    


    <!-- http://purl.obolibrary.org/obo/GAZ_02000361 -->

    <owl:Class rdf:about="http://purl.obolibrary.org/obo/GAZ_02000361">
        <rdfs:subClassOf rdf:resource="http://purl.obolibrary.org/obo/GAZ_00009519"/>
    </owl:Class>
    


    <!-- http://purl.obolibrary.org/obo/GAZ_02000362 -->

    <owl:Class rdf:about="http://purl.obolibrary.org/obo/GAZ_02000362">
        <rdfs:subClassOf rdf:resource="http://purl.obolibrary.org/obo/GAZ_00009519"/>
    </owl:Class>
    


    <!-- http://purl.obolibrary.org/obo/GAZ_02000613 -->

    <owl:Class rdf:about="http://purl.obolibrary.org/obo/GAZ_02000613">
        <rdfs:subClassOf rdf:resource="http://purl.obolibrary.org/obo/GAZ_00004491"/>
    </owl:Class>
    


    <!-- http://purl.obolibrary.org/obo/GAZ_02000614 -->

    <owl:Class rdf:about="http://purl.obolibrary.org/obo/GAZ_02000614">
        <rdfs:subClassOf rdf:resource="http://purl.obolibrary.org/obo/GAZ_00004491"/>
    </owl:Class>
    


    <!-- http://purl.obolibrary.org/obo/GAZ_02000615 -->

    <owl:Class rdf:about="http://purl.obolibrary.org/obo/GAZ_02000615">
        <rdfs:subClassOf rdf:resource="http://purl.obolibrary.org/obo/GAZ_00004491"/>
    </owl:Class>
    


    <!-- http://purl.obolibrary.org/obo/GAZ_02000616 -->

    <owl:Class rdf:about="http://purl.obolibrary.org/obo/GAZ_02000616">
        <rdfs:subClassOf rdf:resource="http://purl.obolibrary.org/obo/GAZ_00004491"/>
    </owl:Class>
    


    <!-- http://purl.obolibrary.org/obo/GAZ_02000617 -->

    <owl:Class rdf:about="http://purl.obolibrary.org/obo/GAZ_02000617">
        <rdfs:subClassOf rdf:resource="http://purl.obolibrary.org/obo/GAZ_00004491"/>
    </owl:Class>
    


    <!-- http://purl.obolibrary.org/obo/GAZ_02000618 -->

    <owl:Class rdf:about="http://purl.obolibrary.org/obo/GAZ_02000618">
        <rdfs:subClassOf rdf:resource="http://purl.obolibrary.org/obo/GAZ_00004491"/>
    </owl:Class>
    


    <!-- http://purl.obolibrary.org/obo/GAZ_02000619 -->

    <owl:Class rdf:about="http://purl.obolibrary.org/obo/GAZ_02000619">
        <rdfs:subClassOf rdf:resource="http://purl.obolibrary.org/obo/GAZ_00004491"/>
    </owl:Class>
    


    <!-- http://purl.obolibrary.org/obo/GAZ_02000620 -->

    <owl:Class rdf:about="http://purl.obolibrary.org/obo/GAZ_02000620">
        <rdfs:subClassOf rdf:resource="http://purl.obolibrary.org/obo/GAZ_00004491"/>
    </owl:Class>
    


    <!-- http://purl.obolibrary.org/obo/GAZ_02000621 -->

    <owl:Class rdf:about="http://purl.obolibrary.org/obo/GAZ_02000621">
        <rdfs:subClassOf rdf:resource="http://purl.obolibrary.org/obo/GAZ_00004491"/>
    </owl:Class>
    


    <!-- http://purl.obolibrary.org/obo/GAZ_02000622 -->

    <owl:Class rdf:about="http://purl.obolibrary.org/obo/GAZ_02000622">
        <rdfs:subClassOf rdf:resource="http://purl.obolibrary.org/obo/GAZ_00004491"/>
    </owl:Class>
    


    <!-- http://purl.obolibrary.org/obo/GAZ_02000623 -->

    <owl:Class rdf:about="http://purl.obolibrary.org/obo/GAZ_02000623">
        <rdfs:subClassOf rdf:resource="http://purl.obolibrary.org/obo/GAZ_00004491"/>
    </owl:Class>
    


    <!-- http://purl.obolibrary.org/obo/GAZ_02000624 -->

    <owl:Class rdf:about="http://purl.obolibrary.org/obo/GAZ_02000624">
        <rdfs:subClassOf rdf:resource="http://purl.obolibrary.org/obo/GAZ_00004491"/>
    </owl:Class>
    


    <!-- http://purl.obolibrary.org/obo/GAZ_02000625 -->

    <owl:Class rdf:about="http://purl.obolibrary.org/obo/GAZ_02000625">
        <rdfs:subClassOf rdf:resource="http://purl.obolibrary.org/obo/GAZ_00004491"/>
    </owl:Class>
    


    <!-- http://purl.obolibrary.org/obo/GAZ_02000626 -->

    <owl:Class rdf:about="http://purl.obolibrary.org/obo/GAZ_02000626">
        <rdfs:subClassOf rdf:resource="http://purl.obolibrary.org/obo/GAZ_00004491"/>
    </owl:Class>
    


    <!-- http://purl.obolibrary.org/obo/GAZ_02000627 -->

    <owl:Class rdf:about="http://purl.obolibrary.org/obo/GAZ_02000627">
        <rdfs:subClassOf rdf:resource="http://purl.obolibrary.org/obo/GAZ_00004491"/>
    </owl:Class>
    


    <!-- 
    ///////////////////////////////////////////////////////////////////////////////////////
    //
    // Individuals
    //
    ///////////////////////////////////////////////////////////////////////////////////////
     -->

    


    <!-- http://purl.obolibrary.org/obo/GAZ_00004481 -->

    <owl:NamedIndividual rdf:about="http://purl.obolibrary.org/obo/GAZ_00004481">
        <obo:IAO_0000115>A mountain range that has a total length of 1 500 km from western Iran, specifically South Kurdistan (Northern Iraq) region on the border with Iraq to the southern parts of the Persian Gulf. The mountain range ends at the Straits of Hormuz.</obo:IAO_0000115>
        <oboInOwl:hasOBONamespace>GAZ</oboInOwl:hasOBONamespace>
        <oboInOwl:id>GAZ:00004481</oboInOwl:id>
        <rdfs:label>Zagros Mountains</rdfs:label>
    </owl:NamedIndividual>
    


    <!-- http://purl.obolibrary.org/obo/GAZ_00004482 -->

    <owl:NamedIndividual rdf:about="http://purl.obolibrary.org/obo/GAZ_00004482">
        <obo:RO_0001025 rdf:resource="http://purl.obolibrary.org/obo/GAZ_00004481"/>
        <oboInOwl:hasOBONamespace>GAZ</oboInOwl:hasOBONamespace>
        <oboInOwl:id>GAZ:00004482</oboInOwl:id>
        <rdfs:label>Mount Dena</rdfs:label>
    </owl:NamedIndividual>
    


    <!-- http://purl.obolibrary.org/obo/GAZ_00004483 -->

    <owl:NamedIndividual rdf:about="http://purl.obolibrary.org/obo/GAZ_00004483">
        <rdf:type rdf:resource="http://purl.obolibrary.org/obo/ENVO_00000009"/>
        <obo:IAO_0000115>A country in the Middle East spanning most of the northwestern end of the Zagros mountain range, the eastern part of the Syrian Desert and the northern part of the Arabian Desert. It shares borders with Kuwait and Saudi Arabia to the south, Jordan to the west, Syria to the northwest, Turkey to the north, and Iran to the east. It has a very narrow section of coastline at Umm Qasr on the Persian Gulf. There are two major flowing rivers: the Tigris and the Euphrates. Iraq is divided into 18 governorates (or provinces) (muhafazah). The governorates are divided into qadhas (or districts).</obo:IAO_0000115>
        <oboInOwl:hasOBONamespace>GAZ</oboInOwl:hasOBONamespace>
        <oboInOwl:id>GAZ:00004483</oboInOwl:id>
        <rdfs:label>Iraq</rdfs:label>
    </owl:NamedIndividual>
    


    <!-- http://purl.obolibrary.org/obo/GAZ_00004491 -->

    <owl:NamedIndividual rdf:about="http://purl.obolibrary.org/obo/GAZ_00004491">
        <obo:RO_0001025 rdf:resource="http://purl.obolibrary.org/obo/GAZ_00004483"/>
    </owl:NamedIndividual>
    


    <!-- http://purl.obolibrary.org/obo/GAZ_00004492 -->

    <owl:NamedIndividual rdf:about="http://purl.obolibrary.org/obo/GAZ_00004492"/>
    


    <!-- http://purl.obolibrary.org/obo/GAZ_00004493 -->

    <owl:NamedIndividual rdf:about="http://purl.obolibrary.org/obo/GAZ_00004493">
        <obo:RO_0001025 rdf:resource="http://purl.obolibrary.org/obo/GAZ_00030439"/>
    </owl:NamedIndividual>
    


    <!-- http://purl.obolibrary.org/obo/GAZ_00004494 -->

    <owl:NamedIndividual rdf:about="http://purl.obolibrary.org/obo/GAZ_00004494">
        <obo:RO_0001025 rdf:resource="http://purl.obolibrary.org/obo/GAZ_00004493"/>
        <oboInOwl:hasOBONamespace>GAZ</oboInOwl:hasOBONamespace>
        <oboInOwl:id>GAZ:00004494</oboInOwl:id>
        <rdfs:label>Saraji Park</rdfs:label>
    </owl:NamedIndividual>
    


    <!-- http://purl.obolibrary.org/obo/GAZ_00004495 -->

    <owl:NamedIndividual rdf:about="http://purl.obolibrary.org/obo/GAZ_00004495">
        <obo:RO_0001025 rdf:resource="http://purl.obolibrary.org/obo/GAZ_00004483"/>
    </owl:NamedIndividual>
    


    <!-- http://purl.obolibrary.org/obo/GAZ_00005281 -->

    <owl:NamedIndividual rdf:about="http://purl.obolibrary.org/obo/GAZ_00005281">
        <obo:RO_0001025 rdf:resource="http://purl.obolibrary.org/obo/GAZ_00006936"/>
        <obo:IAO_0000115>A borderless island country in the Persian Gulf. Saudi Arabia lies to the west and is connected to Bahrain by the King Fahd Causeway, and Qatar is to the south across the Gulf of Bahrain. Bahrain is split into five governorates.</obo:IAO_0000115>
        <oboInOwl:hasOBONamespace>GAZ</oboInOwl:hasOBONamespace>
        <oboInOwl:id>GAZ:00005281</oboInOwl:id>
        <rdfs:label>Bahrain</rdfs:label>
    </owl:NamedIndividual>
    


    <!-- http://purl.obolibrary.org/obo/GAZ_00005295 -->

    <owl:NamedIndividual rdf:about="http://purl.obolibrary.org/obo/GAZ_00005295">
        <obo:IAO_0000115>A gulf bounded by the coasts of Oman, United Arab Emirates, Qatar, Saudi Arabia, Kuwait, Irak and Iran. Its southeastern limit with the Gulf of Oman (in the Strait of Hormuz) is the following: A line joining Cape L Degrees mah (25 Degrees 56 Minutes 35 Seconds N - 56 Degrees 27 Minutes 30 Seconds E), in Oman, eastward to Cape Al K Degrees h (25 Degrees 47 Minutes 30 Seconds N - 57 Degrees 18 Minutes E), in Iran.</obo:IAO_0000115>
        <oboInOwl:hasOBONamespace>GAZ</oboInOwl:hasOBONamespace>
        <oboInOwl:id>GAZ:00005295</oboInOwl:id>
        <rdfs:label>Persian Gulf</rdfs:label>
    </owl:NamedIndividual>
    


    <!-- http://purl.obolibrary.org/obo/GAZ_00006936 -->

    <owl:NamedIndividual rdf:about="http://purl.obolibrary.org/obo/GAZ_00006936">
        <obo:RO_0001025 rdf:resource="http://purl.obolibrary.org/obo/GAZ_00005295"/>
        <oboInOwl:hasOBONamespace>GAZ</oboInOwl:hasOBONamespace>
        <oboInOwl:id>GAZ:00006936</oboInOwl:id>
        <rdfs:label>Bahrain Archipelago</rdfs:label>
    </owl:NamedIndividual>
    


    <!-- http://purl.obolibrary.org/obo/GAZ_00006937 -->

    <owl:NamedIndividual rdf:about="http://purl.obolibrary.org/obo/GAZ_00006937">
        <obo:RO_0001025 rdf:resource="http://purl.obolibrary.org/obo/GAZ_00006936"/>
        <oboInOwl:hasOBONamespace>GAZ</oboInOwl:hasOBONamespace>
        <oboInOwl:id>GAZ:00006937</oboInOwl:id>
        <rdfs:label>Bahrain Island</rdfs:label>
    </owl:NamedIndividual>
    


    <!-- http://purl.obolibrary.org/obo/GAZ_00006938 -->

    <owl:NamedIndividual rdf:about="http://purl.obolibrary.org/obo/GAZ_00006938">
        <obo:RO_0001025 rdf:resource="http://purl.obolibrary.org/obo/GAZ_00006936"/>
        <oboInOwl:hasOBONamespace>GAZ</oboInOwl:hasOBONamespace>
        <oboInOwl:id>GAZ:00006938</oboInOwl:id>
        <rdfs:label>Al Muharraq</rdfs:label>
    </owl:NamedIndividual>
    


    <!-- http://purl.obolibrary.org/obo/GAZ_00006939 -->

    <owl:NamedIndividual rdf:about="http://purl.obolibrary.org/obo/GAZ_00006939">
        <obo:RO_0001025 rdf:resource="http://purl.obolibrary.org/obo/GAZ_00006936"/>
        <oboInOwl:hasOBONamespace>GAZ</oboInOwl:hasOBONamespace>
        <oboInOwl:id>GAZ:00006939</oboInOwl:id>
        <rdfs:label>Jazirat al Azl</rdfs:label>
    </owl:NamedIndividual>
    


    <!-- http://purl.obolibrary.org/obo/GAZ_00006940 -->

    <owl:NamedIndividual rdf:about="http://purl.obolibrary.org/obo/GAZ_00006940">
        <obo:RO_0001025 rdf:resource="http://purl.obolibrary.org/obo/GAZ_00006936"/>
        <oboInOwl:hasOBONamespace>GAZ</oboInOwl:hasOBONamespace>
        <oboInOwl:id>GAZ:00006940</oboInOwl:id>
        <rdfs:label>Sitrah</rdfs:label>
    </owl:NamedIndividual>
    


    <!-- http://purl.obolibrary.org/obo/GAZ_00006941 -->

    <owl:NamedIndividual rdf:about="http://purl.obolibrary.org/obo/GAZ_00006941">
        <obo:RO_0001025 rdf:resource="http://purl.obolibrary.org/obo/GAZ_00006936"/>
        <oboInOwl:hasOBONamespace>GAZ</oboInOwl:hasOBONamespace>
        <oboInOwl:id>GAZ:00006941</oboInOwl:id>
        <rdfs:label>Umm an Nasan</rdfs:label>
    </owl:NamedIndividual>
    


    <!-- http://purl.obolibrary.org/obo/GAZ_00006942 -->

    <owl:NamedIndividual rdf:about="http://purl.obolibrary.org/obo/GAZ_00006942">
        <obo:RO_0001025 rdf:resource="http://purl.obolibrary.org/obo/GAZ_00006936"/>
        <obo:RO_0001025 rdf:resource="http://purl.obolibrary.org/obo/GAZ_00124888"/>
        <obo:IAO_0000115>An island in Bahrain. It lies in the Tubli Bay, east of Bahrain Island. It is connected to Bahrain Island and Sitra through the Sitra Causeway.</obo:IAO_0000115>
        <oboInOwl:hasOBONamespace>GAZ</oboInOwl:hasOBONamespace>
        <oboInOwl:id>GAZ:00006942</oboInOwl:id>
        <rdfs:label>Nabi Salah</rdfs:label>
    </owl:NamedIndividual>
    


    <!-- http://purl.obolibrary.org/obo/GAZ_00006943 -->

    <owl:NamedIndividual rdf:about="http://purl.obolibrary.org/obo/GAZ_00006943">
        <obo:RO_0001025 rdf:resource="http://purl.obolibrary.org/obo/GAZ_00006936"/>
        <oboInOwl:hasOBONamespace>GAZ</oboInOwl:hasOBONamespace>
        <oboInOwl:id>GAZ:00006943</oboInOwl:id>
        <rdfs:label>Jiddah</rdfs:label>
    </owl:NamedIndividual>
    


    <!-- http://purl.obolibrary.org/obo/GAZ_00006944 -->

    <owl:NamedIndividual rdf:about="http://purl.obolibrary.org/obo/GAZ_00006944">
        <obo:RO_0001025 rdf:resource="http://purl.obolibrary.org/obo/GAZ_00078661"/>
        <obo:IAO_0000115>The largest of the Hawar Islands of Bahrain.</obo:IAO_0000115>
        <oboInOwl:hasOBONamespace>GAZ</oboInOwl:hasOBONamespace>
        <oboInOwl:id>GAZ:00006944</oboInOwl:id>
        <rdfs:label>Hawar</rdfs:label>
    </owl:NamedIndividual>
    


    <!-- http://purl.obolibrary.org/obo/GAZ_00006945 -->

    <owl:NamedIndividual rdf:about="http://purl.obolibrary.org/obo/GAZ_00006945">
        <obo:RO_0001025 rdf:resource="http://purl.obolibrary.org/obo/GAZ_00006936"/>
        <obo:IAO_0000115>A group of man-made islands located in the northeast of Bahrain, near the coast of Muharraq island.</obo:IAO_0000115>
        <oboInOwl:hasOBONamespace>GAZ</oboInOwl:hasOBONamespace>
        <oboInOwl:id>GAZ:00006945</oboInOwl:id>
        <rdfs:label>Amwaj Islands</rdfs:label>
    </owl:NamedIndividual>
    


    <!-- http://purl.obolibrary.org/obo/GAZ_00006946 -->

    <owl:NamedIndividual rdf:about="http://purl.obolibrary.org/obo/GAZ_00006946">
        <obo:RO_0001025 rdf:resource="http://purl.obolibrary.org/obo/GAZ_00005295"/>
        <obo:IAO_0000115>An island in the Persian Gulf. It extends from Ras Tanura in the north to Qatif in the west. It also is connected to Qatif by two causeways.</obo:IAO_0000115>
        <oboInOwl:hasOBONamespace>GAZ</oboInOwl:hasOBONamespace>
        <oboInOwl:id>GAZ:00006946</oboInOwl:id>
        <rdfs:label>Tarout Island</rdfs:label>
    </owl:NamedIndividual>
    


    <!-- http://purl.obolibrary.org/obo/GAZ_00009519 -->

    <owl:NamedIndividual rdf:about="http://purl.obolibrary.org/obo/GAZ_00009519">
        <obo:RO_0001025 rdf:resource="http://purl.obolibrary.org/obo/GAZ_00005281"/>
    </owl:NamedIndividual>
    


    <!-- http://purl.obolibrary.org/obo/GAZ_00010359 -->

    <owl:NamedIndividual rdf:about="http://purl.obolibrary.org/obo/GAZ_00010359"/>
    


    <!-- http://purl.obolibrary.org/obo/GAZ_00010360 -->

    <owl:NamedIndividual rdf:about="http://purl.obolibrary.org/obo/GAZ_00010360">
        <obo:RO_0001025 rdf:resource="http://purl.obolibrary.org/obo/GAZ_00251083"/>
    </owl:NamedIndividual>
    


    <!-- http://purl.obolibrary.org/obo/GAZ_00018501 -->

    <owl:NamedIndividual rdf:about="http://purl.obolibrary.org/obo/GAZ_00018501">
        <obo:RO_0001025 rdf:resource="http://purl.obolibrary.org/obo/GAZ_00005295"/>
        <oboInOwl:hasOBONamespace>GAZ</oboInOwl:hasOBONamespace>
        <oboInOwl:id>GAZ:00018501</oboInOwl:id>
        <rdfs:label>Kuwait Bay</rdfs:label>
    </owl:NamedIndividual>
    


    <!-- http://purl.obolibrary.org/obo/GAZ_00018502 -->

    <owl:NamedIndividual rdf:about="http://purl.obolibrary.org/obo/GAZ_00018502">
        <obo:RO_0001025 rdf:resource="http://purl.obolibrary.org/obo/GAZ_00005295"/>
        <obo:IAO_0000115>An island in the Persian Gulf.</obo:IAO_0000115>
        <oboInOwl:hasOBONamespace>GAZ</oboInOwl:hasOBONamespace>
        <oboInOwl:id>GAZ:00018502</oboInOwl:id>
        <rdfs:label>Shomali Island</rdfs:label>
    </owl:NamedIndividual>
    


    <!-- http://purl.obolibrary.org/obo/GAZ_00018503 -->

    <owl:NamedIndividual rdf:about="http://purl.obolibrary.org/obo/GAZ_00018503">
        <obo:RO_0001025 rdf:resource="http://purl.obolibrary.org/obo/GAZ_00005295"/>
        <obo:IAO_0000115>An island in the Persian Gulf.</obo:IAO_0000115>
        <oboInOwl:hasOBONamespace>GAZ</oboInOwl:hasOBONamespace>
        <oboInOwl:id>GAZ:00018503</oboInOwl:id>
        <rdfs:label>Smaller Bent Island</rdfs:label>
    </owl:NamedIndividual>
    


    <!-- http://purl.obolibrary.org/obo/GAZ_00018504 -->

    <owl:NamedIndividual rdf:about="http://purl.obolibrary.org/obo/GAZ_00018504">
        <obo:RO_0001025 rdf:resource="http://purl.obolibrary.org/obo/GAZ_00005295"/>
        <obo:IAO_0000115>An island situated in the Strait of Hormuz off the south coast of Iran and east of the Persian Gulf.</obo:IAO_0000115>
        <oboInOwl:hasOBONamespace>GAZ</oboInOwl:hasOBONamespace>
        <oboInOwl:id>GAZ:00018504</oboInOwl:id>
        <rdfs:label>Qeshm Island</rdfs:label>
    </owl:NamedIndividual>
    


    <!-- http://purl.obolibrary.org/obo/GAZ_00018505 -->

    <owl:NamedIndividual rdf:about="http://purl.obolibrary.org/obo/GAZ_00018505">
        <obo:RO_0001025 rdf:resource="http://purl.obolibrary.org/obo/GAZ_00005295"/>
        <obo:IAO_0000115>An island in the Persian Gulf.</obo:IAO_0000115>
        <oboInOwl:hasOBONamespace>GAZ</oboInOwl:hasOBONamespace>
        <oboInOwl:id>GAZ:00018505</oboInOwl:id>
        <rdfs:label>Shatvar Island</rdfs:label>
    </owl:NamedIndividual>
    


    <!-- http://purl.obolibrary.org/obo/GAZ_00018506 -->

    <owl:NamedIndividual rdf:about="http://purl.obolibrary.org/obo/GAZ_00018506">
        <obo:RO_0001025 rdf:resource="http://purl.obolibrary.org/obo/GAZ_00005295"/>
        <obo:IAO_0000115>An island in the Persian Gulf.</obo:IAO_0000115>
        <oboInOwl:hasOBONamespace>GAZ</oboInOwl:hasOBONamespace>
        <oboInOwl:id>GAZ:00018506</oboInOwl:id>
        <rdfs:label>Shetor Island</rdfs:label>
    </owl:NamedIndividual>
    


    <!-- http://purl.obolibrary.org/obo/GAZ_00018507 -->

    <owl:NamedIndividual rdf:about="http://purl.obolibrary.org/obo/GAZ_00018507">
        <obo:RO_0001025 rdf:resource="http://purl.obolibrary.org/obo/GAZ_00005295"/>
        <obo:IAO_0000115>An island in the Persian Gulf.</obo:IAO_0000115>
        <oboInOwl:hasOBONamespace>GAZ</oboInOwl:hasOBONamespace>
        <oboInOwl:id>GAZ:00018507</oboInOwl:id>
        <rdfs:label>Qabre Nakhoda Island</rdfs:label>
    </owl:NamedIndividual>
    


    <!-- http://purl.obolibrary.org/obo/GAZ_00018508 -->

    <owl:NamedIndividual rdf:about="http://purl.obolibrary.org/obo/GAZ_00018508">
        <obo:RO_0001025 rdf:resource="http://purl.obolibrary.org/obo/GAZ_00005295"/>
        <obo:IAO_0000115>An island in the Persian Gulf.</obo:IAO_0000115>
        <oboInOwl:hasOBONamespace>GAZ</oboInOwl:hasOBONamespace>
        <oboInOwl:id>GAZ:00018508</oboInOwl:id>
        <rdfs:label>Rostam Island</rdfs:label>
    </owl:NamedIndividual>
    


    <!-- http://purl.obolibrary.org/obo/GAZ_00018509 -->

    <owl:NamedIndividual rdf:about="http://purl.obolibrary.org/obo/GAZ_00018509">
        <obo:RO_0001025 rdf:resource="http://purl.obolibrary.org/obo/GAZ_00250913"/>
        <obo:IAO_0000115>An island in the Persian Gulf.</obo:IAO_0000115>
        <oboInOwl:hasOBONamespace>GAZ</oboInOwl:hasOBONamespace>
        <oboInOwl:id>GAZ:00018509</oboInOwl:id>
        <rdfs:label>Shif Island</rdfs:label>
    </owl:NamedIndividual>
    


    <!-- http://purl.obolibrary.org/obo/GAZ_00018510 -->

    <owl:NamedIndividual rdf:about="http://purl.obolibrary.org/obo/GAZ_00018510">
        <obo:RO_0001025 rdf:resource="http://purl.obolibrary.org/obo/GAZ_00005295"/>
        <obo:IAO_0000115>An island in the Persian Gulf.</obo:IAO_0000115>
        <oboInOwl:hasOBONamespace>GAZ</oboInOwl:hasOBONamespace>
        <oboInOwl:id>GAZ:00018510</oboInOwl:id>
        <rdfs:label>Sirri Island</rdfs:label>
    </owl:NamedIndividual>
    


    <!-- http://purl.obolibrary.org/obo/GAZ_00018511 -->

    <owl:NamedIndividual rdf:about="http://purl.obolibrary.org/obo/GAZ_00018511">
        <obo:RO_0001025 rdf:resource="http://purl.obolibrary.org/obo/GAZ_00005295"/>
        <obo:IAO_0000115>An island in the Persian Gulf.</obo:IAO_0000115>
        <oboInOwl:hasOBONamespace>GAZ</oboInOwl:hasOBONamespace>
        <oboInOwl:id>GAZ:00018511</oboInOwl:id>
        <rdfs:label>Jonobi Island</rdfs:label>
    </owl:NamedIndividual>
    


    <!-- http://purl.obolibrary.org/obo/GAZ_00018512 -->

    <owl:NamedIndividual rdf:about="http://purl.obolibrary.org/obo/GAZ_00018512">
        <obo:RO_0001025 rdf:resource="http://purl.obolibrary.org/obo/GAZ_00005295"/>
        <obo:IAO_0000115>An Iranian island in the Persian Gulf.</obo:IAO_0000115>
        <oboInOwl:hasOBONamespace>GAZ</oboInOwl:hasOBONamespace>
        <oboInOwl:id>GAZ:00018512</oboInOwl:id>
        <rdfs:label>Farsi Island</rdfs:label>
    </owl:NamedIndividual>
    


    <!-- http://purl.obolibrary.org/obo/GAZ_00018513 -->

    <owl:NamedIndividual rdf:about="http://purl.obolibrary.org/obo/GAZ_00018513">
        <obo:RO_0001025 rdf:resource="http://purl.obolibrary.org/obo/GAZ_00250921"/>
        <obo:IAO_0000115>An island in the Persian Gulf.</obo:IAO_0000115>
        <oboInOwl:hasOBONamespace>GAZ</oboInOwl:hasOBONamespace>
        <oboInOwl:id>GAZ:00018513</oboInOwl:id>
        <rdfs:label>Jazireh-ye Forur</rdfs:label>
    </owl:NamedIndividual>
    


    <!-- http://purl.obolibrary.org/obo/GAZ_00018514 -->

    <owl:NamedIndividual rdf:about="http://purl.obolibrary.org/obo/GAZ_00018514">
        <obo:RO_0001025 rdf:resource="http://purl.obolibrary.org/obo/GAZ_00005295"/>
        <obo:IAO_0000115>A resort island in the Persian Gulf. It is part of the Hormozgan Province of Iran.</obo:IAO_0000115>
        <oboInOwl:hasOBONamespace>GAZ</oboInOwl:hasOBONamespace>
        <oboInOwl:id>GAZ:00018514</oboInOwl:id>
        <rdfs:label>Kish Island</rdfs:label>
    </owl:NamedIndividual>
    


    <!-- http://purl.obolibrary.org/obo/GAZ_00018515 -->

    <owl:NamedIndividual rdf:about="http://purl.obolibrary.org/obo/GAZ_00018515">
        <obo:RO_0001025 rdf:resource="http://purl.obolibrary.org/obo/GAZ_00005295"/>
        <obo:IAO_0000115>An island off the coast of Iran in the Persian Gulf.</obo:IAO_0000115>
        <oboInOwl:hasOBONamespace>GAZ</oboInOwl:hasOBONamespace>
        <oboInOwl:id>GAZ:00018515</oboInOwl:id>
        <rdfs:label>Larak Island</rdfs:label>
    </owl:NamedIndividual>
    


    <!-- http://purl.obolibrary.org/obo/GAZ_00018516 -->

    <owl:NamedIndividual rdf:about="http://purl.obolibrary.org/obo/GAZ_00018516">
        <obo:RO_0001025 rdf:resource="http://purl.obolibrary.org/obo/GAZ_00005295"/>
        <obo:IAO_0000115>An Iranian island in the Persian Gulf.</obo:IAO_0000115>
        <oboInOwl:hasOBONamespace>GAZ</oboInOwl:hasOBONamespace>
        <oboInOwl:id>GAZ:00018516</oboInOwl:id>
        <rdfs:label>Lavan Island</rdfs:label>
    </owl:NamedIndividual>
    


    <!-- http://purl.obolibrary.org/obo/GAZ_00018517 -->

    <owl:NamedIndividual rdf:about="http://purl.obolibrary.org/obo/GAZ_00018517">
        <obo:RO_0001025 rdf:resource="http://purl.obolibrary.org/obo/GAZ_00005295"/>
        <obo:IAO_0000115>A continental island in the Persian Gulf belonging to Iran.</obo:IAO_0000115>
        <oboInOwl:hasOBONamespace>GAZ</oboInOwl:hasOBONamespace>
        <oboInOwl:id>GAZ:00018517</oboInOwl:id>
        <rdfs:label>Kharg Island</rdfs:label>
    </owl:NamedIndividual>
    


    <!-- http://purl.obolibrary.org/obo/GAZ_00018518 -->

    <owl:NamedIndividual rdf:about="http://purl.obolibrary.org/obo/GAZ_00018518">
        <obo:RO_0001025 rdf:resource="http://purl.obolibrary.org/obo/GAZ_00005295"/>
        <obo:IAO_0000115>An Iranian island in the Persian Gulf. It is part of the Khuzestan province in southwestern Iran and is close to the city of Abadan.</obo:IAO_0000115>
        <oboInOwl:hasOBONamespace>GAZ</oboInOwl:hasOBONamespace>
        <oboInOwl:id>GAZ:00018518</oboInOwl:id>
        <rdfs:label>Minu Island</rdfs:label>
    </owl:NamedIndividual>
    


    <!-- http://purl.obolibrary.org/obo/GAZ_00018519 -->

    <owl:NamedIndividual rdf:about="http://purl.obolibrary.org/obo/GAZ_00018519">
        <obo:RO_0001025 rdf:resource="http://purl.obolibrary.org/obo/GAZ_00005295"/>
        <obo:IAO_0000115>An island in the Persian Gulf.</obo:IAO_0000115>
        <oboInOwl:hasOBONamespace>GAZ</oboInOwl:hasOBONamespace>
        <oboInOwl:id>GAZ:00018519</oboInOwl:id>
        <rdfs:label>Omolkarm Island</rdfs:label>
    </owl:NamedIndividual>
    


    <!-- http://purl.obolibrary.org/obo/GAZ_00018520 -->

    <owl:NamedIndividual rdf:about="http://purl.obolibrary.org/obo/GAZ_00018520">
        <obo:RO_0001025 rdf:resource="http://purl.obolibrary.org/obo/GAZ_00005295"/>
        <obo:IAO_0000115>An island.</obo:IAO_0000115>
        <oboInOwl:hasOBONamespace>GAZ</oboInOwl:hasOBONamespace>
        <oboInOwl:id>GAZ:00018520</oboInOwl:id>
        <rdfs:label>Dara Island</rdfs:label>
    </owl:NamedIndividual>
    


    <!-- http://purl.obolibrary.org/obo/GAZ_00018521 -->

    <owl:NamedIndividual rdf:about="http://purl.obolibrary.org/obo/GAZ_00018521">
        <obo:RO_0001025 rdf:resource="http://purl.obolibrary.org/obo/GAZ_00005295"/>
        <obo:IAO_0000115>An island located on the eastern side of the Persian Gulf, part of a six-island archipelago near the entrance to the Strait of Hormuz.</obo:IAO_0000115>
        <oboInOwl:hasOBONamespace>GAZ</oboInOwl:hasOBONamespace>
        <oboInOwl:id>GAZ:00018521</oboInOwl:id>
        <rdfs:label>Abu Musa Island</rdfs:label>
    </owl:NamedIndividual>
    


    <!-- http://purl.obolibrary.org/obo/GAZ_00018522 -->

    <owl:NamedIndividual rdf:about="http://purl.obolibrary.org/obo/GAZ_00018522">
        <obo:RO_0001025 rdf:resource="http://purl.obolibrary.org/obo/GAZ_00005295"/>
        <oboInOwl:hasOBONamespace>GAZ</oboInOwl:hasOBONamespace>
        <oboInOwl:id>GAZ:00018522</oboInOwl:id>
        <rdfs:label>Abbasak Island</rdfs:label>
    </owl:NamedIndividual>
    


    <!-- http://purl.obolibrary.org/obo/GAZ_00018523 -->

    <owl:NamedIndividual rdf:about="http://purl.obolibrary.org/obo/GAZ_00018523">
        <obo:RO_0001025 rdf:resource="http://purl.obolibrary.org/obo/GAZ_00005295"/>
        <obo:IAO_0000115>An island in the N Persian Gulf.</obo:IAO_0000115>
        <oboInOwl:hasOBONamespace>GAZ</oboInOwl:hasOBONamespace>
        <oboInOwl:id>GAZ:00018523</oboInOwl:id>
        <rdfs:label>Buneh Island</rdfs:label>
    </owl:NamedIndividual>
    


    <!-- http://purl.obolibrary.org/obo/GAZ_00018524 -->

    <owl:NamedIndividual rdf:about="http://purl.obolibrary.org/obo/GAZ_00018524">
        <obo:RO_0001025 rdf:resource="http://purl.obolibrary.org/obo/GAZ_00005295"/>
        <obo:IAO_0000115>An island located in the straight of Hormuz and is part of the Hormozgan Province.</obo:IAO_0000115>
        <oboInOwl:hasOBONamespace>GAZ</oboInOwl:hasOBONamespace>
        <oboInOwl:id>GAZ:00018524</oboInOwl:id>
        <rdfs:label>Hormuz Island</rdfs:label>
    </owl:NamedIndividual>
    


    <!-- http://purl.obolibrary.org/obo/GAZ_00018525 -->

    <owl:NamedIndividual rdf:about="http://purl.obolibrary.org/obo/GAZ_00018525">
        <obo:RO_0001025 rdf:resource="http://purl.obolibrary.org/obo/GAZ_00005295"/>
        <obo:IAO_0000115>Two small islands in the eastern Persian Gulf, close to the Strait of Hormuz, some 12 km from each other and 20 south of the Iranian island of Qeshm.</obo:IAO_0000115>
        <oboInOwl:hasOBONamespace>GAZ</oboInOwl:hasOBONamespace>
        <oboInOwl:id>GAZ:00018525</oboInOwl:id>
        <rdfs:label>Greater and Lesser Tunbs</rdfs:label>
    </owl:NamedIndividual>
    


    <!-- http://purl.obolibrary.org/obo/GAZ_00018526 -->

    <owl:NamedIndividual rdf:about="http://purl.obolibrary.org/obo/GAZ_00018526">
        <obo:RO_0001025 rdf:resource="http://purl.obolibrary.org/obo/GAZ_00005295"/>
        <obo:IAO_0000115>An island in the Persian Gulf, located in Hormozgan Province, to the west of Kish Island and due south of Bastak.</obo:IAO_0000115>
        <oboInOwl:hasOBONamespace>GAZ</oboInOwl:hasOBONamespace>
        <oboInOwl:id>GAZ:00018526</oboInOwl:id>
        <rdfs:label>Hendurabi Island</rdfs:label>
    </owl:NamedIndividual>
    


    <!-- http://purl.obolibrary.org/obo/GAZ_00018527 -->

    <owl:NamedIndividual rdf:about="http://purl.obolibrary.org/obo/GAZ_00018527">
        <obo:RO_0001025 rdf:resource="http://purl.obolibrary.org/obo/GAZ_00005295"/>
        <obo:IAO_0000115>An island in the Persian Gulf.</obo:IAO_0000115>
        <oboInOwl:hasOBONamespace>GAZ</oboInOwl:hasOBONamespace>
        <oboInOwl:id>GAZ:00018527</oboInOwl:id>
        <rdfs:label>Germ Island</rdfs:label>
    </owl:NamedIndividual>
    


    <!-- http://purl.obolibrary.org/obo/GAZ_00018528 -->

    <owl:NamedIndividual rdf:about="http://purl.obolibrary.org/obo/GAZ_00018528">
        <obo:RO_0001025 rdf:resource="http://purl.obolibrary.org/obo/GAZ_00005295"/>
        <obo:IAO_0000115>An island in the Persian Gulf.</obo:IAO_0000115>
        <oboInOwl:hasOBONamespace>GAZ</oboInOwl:hasOBONamespace>
        <oboInOwl:id>GAZ:00018528</oboInOwl:id>
        <rdfs:label>Hengam Island</rdfs:label>
    </owl:NamedIndividual>
    


    <!-- http://purl.obolibrary.org/obo/GAZ_00018529 -->

    <owl:NamedIndividual rdf:about="http://purl.obolibrary.org/obo/GAZ_00018529">
        <obo:RO_0001025 rdf:resource="http://purl.obolibrary.org/obo/GAZ_00250921"/>
        <obo:IAO_0000115>An island in the Persian Gulf.</obo:IAO_0000115>
        <oboInOwl:hasOBONamespace>GAZ</oboInOwl:hasOBONamespace>
        <oboInOwl:id>GAZ:00018529</oboInOwl:id>
        <rdfs:label>Jazireh-ye Bani Forur</rdfs:label>
    </owl:NamedIndividual>
    


    <!-- http://purl.obolibrary.org/obo/GAZ_00018530 -->

    <owl:NamedIndividual rdf:about="http://purl.obolibrary.org/obo/GAZ_00018530">
        <obo:RO_0001025 rdf:resource="http://purl.obolibrary.org/obo/GAZ_00005295"/>
        <obo:IAO_0000115>An island in the Persian Gulf.</obo:IAO_0000115>
        <oboInOwl:hasOBONamespace>GAZ</oboInOwl:hasOBONamespace>
        <oboInOwl:id>GAZ:00018530</oboInOwl:id>
        <rdfs:label>Forurgan Island</rdfs:label>
    </owl:NamedIndividual>
    


    <!-- http://purl.obolibrary.org/obo/GAZ_00018532 -->

    <owl:NamedIndividual rdf:about="http://purl.obolibrary.org/obo/GAZ_00018532">
        <obo:RO_0001025 rdf:resource="http://purl.obolibrary.org/obo/GAZ_00005295"/>
        <oboInOwl:hasOBONamespace>GAZ</oboInOwl:hasOBONamespace>
        <oboInOwl:id>GAZ:00018532</oboInOwl:id>
        <rdfs:label>Northern mudflat islands</rdfs:label>
    </owl:NamedIndividual>
    


    <!-- http://purl.obolibrary.org/obo/GAZ_00018533 -->

    <owl:NamedIndividual rdf:about="http://purl.obolibrary.org/obo/GAZ_00018533">
        <obo:RO_0001025 rdf:resource="http://purl.obolibrary.org/obo/GAZ_00005295"/>
        <oboInOwl:hasOBONamespace>GAZ</oboInOwl:hasOBONamespace>
        <oboInOwl:id>GAZ:00018533</oboInOwl:id>
        <rdfs:label>Failaka Islands</rdfs:label>
    </owl:NamedIndividual>
    


    <!-- http://purl.obolibrary.org/obo/GAZ_00018534 -->

    <owl:NamedIndividual rdf:about="http://purl.obolibrary.org/obo/GAZ_00018534">
        <obo:RO_0001025 rdf:resource="http://purl.obolibrary.org/obo/GAZ_00005295"/>
        <oboInOwl:hasOBONamespace>GAZ</oboInOwl:hasOBONamespace>
        <oboInOwl:id>GAZ:00018534</oboInOwl:id>
        <rdfs:label>Southern Islands</rdfs:label>
    </owl:NamedIndividual>
    


    <!-- http://purl.obolibrary.org/obo/GAZ_00018535 -->

    <owl:NamedIndividual rdf:about="http://purl.obolibrary.org/obo/GAZ_00018535">
        <obo:RO_0001025 rdf:resource="http://purl.obolibrary.org/obo/GAZ_00018532"/>
        <oboInOwl:hasOBONamespace>GAZ</oboInOwl:hasOBONamespace>
        <oboInOwl:id>GAZ:00018535</oboInOwl:id>
        <rdfs:label>Bubiyan Island</rdfs:label>
    </owl:NamedIndividual>
    


    <!-- http://purl.obolibrary.org/obo/GAZ_00018536 -->

    <owl:NamedIndividual rdf:about="http://purl.obolibrary.org/obo/GAZ_00018536">
        <obo:RO_0001025 rdf:resource="http://purl.obolibrary.org/obo/GAZ_00018532"/>
        <oboInOwl:hasOBONamespace>GAZ</oboInOwl:hasOBONamespace>
        <oboInOwl:id>GAZ:00018536</oboInOwl:id>
        <rdfs:label>Warbah Island</rdfs:label>
    </owl:NamedIndividual>
    


    <!-- http://purl.obolibrary.org/obo/GAZ_00018537 -->

    <owl:NamedIndividual rdf:about="http://purl.obolibrary.org/obo/GAZ_00018537">
        <obo:RO_0001025 rdf:resource="http://purl.obolibrary.org/obo/GAZ_00018533"/>
        <oboInOwl:hasOBONamespace>GAZ</oboInOwl:hasOBONamespace>
        <oboInOwl:id>GAZ:00018537</oboInOwl:id>
        <rdfs:label>Auhah Island</rdfs:label>
    </owl:NamedIndividual>
    


    <!-- http://purl.obolibrary.org/obo/GAZ_00018538 -->

    <owl:NamedIndividual rdf:about="http://purl.obolibrary.org/obo/GAZ_00018538">
        <obo:RO_0001025 rdf:resource="http://purl.obolibrary.org/obo/GAZ_00018533"/>
        <oboInOwl:hasOBONamespace>GAZ</oboInOwl:hasOBONamespace>
        <oboInOwl:id>GAZ:00018538</oboInOwl:id>
        <rdfs:label>Failaka Island</rdfs:label>
    </owl:NamedIndividual>
    


    <!-- http://purl.obolibrary.org/obo/GAZ_00018539 -->

    <owl:NamedIndividual rdf:about="http://purl.obolibrary.org/obo/GAZ_00018539">
        <obo:RO_0001025 rdf:resource="http://purl.obolibrary.org/obo/GAZ_00018533"/>
        <oboInOwl:hasOBONamespace>GAZ</oboInOwl:hasOBONamespace>
        <oboInOwl:id>GAZ:00018539</oboInOwl:id>
        <rdfs:label>Miskan Island</rdfs:label>
    </owl:NamedIndividual>
    


    <!-- http://purl.obolibrary.org/obo/GAZ_00018540 -->

    <owl:NamedIndividual rdf:about="http://purl.obolibrary.org/obo/GAZ_00018540">
        <obo:RO_0001025 rdf:resource="http://purl.obolibrary.org/obo/GAZ_00018501"/>
        <oboInOwl:hasOBONamespace>GAZ</oboInOwl:hasOBONamespace>
        <oboInOwl:id>GAZ:00018540</oboInOwl:id>
        <rdfs:label>Shuwaikh Island</rdfs:label>
    </owl:NamedIndividual>
    


    <!-- http://purl.obolibrary.org/obo/GAZ_00018541 -->

    <owl:NamedIndividual rdf:about="http://purl.obolibrary.org/obo/GAZ_00018541">
        <obo:RO_0001025 rdf:resource="http://purl.obolibrary.org/obo/GAZ_00018501"/>
        <oboInOwl:hasOBONamespace>GAZ</oboInOwl:hasOBONamespace>
        <oboInOwl:id>GAZ:00018541</oboInOwl:id>
        <rdfs:label>Umm an Namil Island</rdfs:label>
    </owl:NamedIndividual>
    


    <!-- http://purl.obolibrary.org/obo/GAZ_00018542 -->

    <owl:NamedIndividual rdf:about="http://purl.obolibrary.org/obo/GAZ_00018542">
        <obo:RO_0001025 rdf:resource="http://purl.obolibrary.org/obo/GAZ_00018534"/>
        <oboInOwl:hasOBONamespace>GAZ</oboInOwl:hasOBONamespace>
        <oboInOwl:id>GAZ:00018542</oboInOwl:id>
        <rdfs:label>Umm al Maradim Island</rdfs:label>
    </owl:NamedIndividual>
    


    <!-- http://purl.obolibrary.org/obo/GAZ_00018543 -->

    <owl:NamedIndividual rdf:about="http://purl.obolibrary.org/obo/GAZ_00018543">
        <obo:RO_0001025 rdf:resource="http://purl.obolibrary.org/obo/GAZ_00018534"/>
        <obo:IAO_0000115>A small offshore island with associated coral reefs in the northern Gulf.</obo:IAO_0000115>
        <oboInOwl:hasOBONamespace>GAZ</oboInOwl:hasOBONamespace>
        <oboInOwl:id>GAZ:00018543</oboInOwl:id>
        <rdfs:label>Kubbar Island</rdfs:label>
    </owl:NamedIndividual>
    


    <!-- http://purl.obolibrary.org/obo/GAZ_00018544 -->

    <owl:NamedIndividual rdf:about="http://purl.obolibrary.org/obo/GAZ_00018544">
        <obo:RO_0001025 rdf:resource="http://purl.obolibrary.org/obo/GAZ_00018534"/>
        <oboInOwl:hasOBONamespace>GAZ</oboInOwl:hasOBONamespace>
        <oboInOwl:id>GAZ:00018544</oboInOwl:id>
        <rdfs:label>Qaruh Island</rdfs:label>
    </owl:NamedIndividual>
    


    <!-- http://purl.obolibrary.org/obo/GAZ_00030439 -->

    <owl:NamedIndividual rdf:about="http://purl.obolibrary.org/obo/GAZ_00030439">
        <obo:RO_0001025 rdf:resource="http://purl.obolibrary.org/obo/GAZ_00004492"/>
        <oboInOwl:hasOBONamespace>GAZ</oboInOwl:hasOBONamespace>
        <oboInOwl:id>GAZ:00030439</oboInOwl:id>
        <rdfs:label>Basrah District</rdfs:label>
    </owl:NamedIndividual>
    


    <!-- http://purl.obolibrary.org/obo/GAZ_00030440 -->

    <owl:NamedIndividual rdf:about="http://purl.obolibrary.org/obo/GAZ_00030440">
        <obo:RO_0001025 rdf:resource="http://purl.obolibrary.org/obo/GAZ_00004492"/>
        <oboInOwl:hasOBONamespace>GAZ</oboInOwl:hasOBONamespace>
        <oboInOwl:id>GAZ:00030440</oboInOwl:id>
        <rdfs:label>Al-Midaina District</rdfs:label>
    </owl:NamedIndividual>
    


    <!-- http://purl.obolibrary.org/obo/GAZ_00030441 -->

    <owl:NamedIndividual rdf:about="http://purl.obolibrary.org/obo/GAZ_00030441">
        <obo:RO_0001025 rdf:resource="http://purl.obolibrary.org/obo/GAZ_00004492"/>
        <oboInOwl:hasOBONamespace>GAZ</oboInOwl:hasOBONamespace>
        <oboInOwl:id>GAZ:00030441</oboInOwl:id>
        <rdfs:label>Al-Zubair District</rdfs:label>
    </owl:NamedIndividual>
    


    <!-- http://purl.obolibrary.org/obo/GAZ_00030442 -->

    <owl:NamedIndividual rdf:about="http://purl.obolibrary.org/obo/GAZ_00030442">
        <obo:RO_0001025 rdf:resource="http://purl.obolibrary.org/obo/GAZ_00004492"/>
        <oboInOwl:hasOBONamespace>GAZ</oboInOwl:hasOBONamespace>
        <oboInOwl:id>GAZ:00030442</oboInOwl:id>
        <rdfs:label>Abu Al-Khaseeb District</rdfs:label>
    </owl:NamedIndividual>
    


    <!-- http://purl.obolibrary.org/obo/GAZ_00030443 -->

    <owl:NamedIndividual rdf:about="http://purl.obolibrary.org/obo/GAZ_00030443">
        <obo:RO_0001025 rdf:resource="http://purl.obolibrary.org/obo/GAZ_00004492"/>
        <oboInOwl:hasOBONamespace>GAZ</oboInOwl:hasOBONamespace>
        <oboInOwl:id>GAZ:00030443</oboInOwl:id>
        <rdfs:label>al-Faw District</rdfs:label>
    </owl:NamedIndividual>
    


    <!-- http://purl.obolibrary.org/obo/GAZ_00030444 -->

    <owl:NamedIndividual rdf:about="http://purl.obolibrary.org/obo/GAZ_00030444">
        <obo:RO_0001025 rdf:resource="http://purl.obolibrary.org/obo/GAZ_00004492"/>
        <oboInOwl:hasOBONamespace>GAZ</oboInOwl:hasOBONamespace>
        <oboInOwl:id>GAZ:00030444</oboInOwl:id>
        <rdfs:label>Shatt Al-Arab District</rdfs:label>
    </owl:NamedIndividual>
    


    <!-- http://purl.obolibrary.org/obo/GAZ_00030445 -->

    <owl:NamedIndividual rdf:about="http://purl.obolibrary.org/obo/GAZ_00030445">
        <obo:RO_0001025 rdf:resource="http://purl.obolibrary.org/obo/GAZ_00004492"/>
        <oboInOwl:hasOBONamespace>GAZ</oboInOwl:hasOBONamespace>
        <oboInOwl:id>GAZ:00030445</oboInOwl:id>
        <rdfs:label>Al-Qurna District</rdfs:label>
    </owl:NamedIndividual>
    


    <!-- http://purl.obolibrary.org/obo/GAZ_00030446 -->

    <owl:NamedIndividual rdf:about="http://purl.obolibrary.org/obo/GAZ_00030446">
        <obo:RO_0001025 rdf:resource="http://purl.obolibrary.org/obo/GAZ_02000627"/>
        <oboInOwl:hasOBONamespace>GAZ</oboInOwl:hasOBONamespace>
        <oboInOwl:id>GAZ:00030446</oboInOwl:id>
        <rdfs:label>Kadhimiya District</rdfs:label>
    </owl:NamedIndividual>
    


    <!-- http://purl.obolibrary.org/obo/GAZ_00030447 -->

    <owl:NamedIndividual rdf:about="http://purl.obolibrary.org/obo/GAZ_00030447">
        <rdf:type rdf:resource="http://purl.obolibrary.org/obo/ENVO_00000004"/>
        <obo:RO_0001025 rdf:resource="http://purl.obolibrary.org/obo/GAZ_02000627"/>
        <obo:IAO_0000115>A district in Al Anbar Governorate, Iraq. It is centered around the city of Fallujah.</obo:IAO_0000115>
        <oboInOwl:hasOBONamespace>GAZ</oboInOwl:hasOBONamespace>
        <oboInOwl:id>GAZ:00030447</oboInOwl:id>
        <rdfs:label>Falluja District</rdfs:label>
    </owl:NamedIndividual>
    


    <!-- http://purl.obolibrary.org/obo/GAZ_00030448 -->

    <owl:NamedIndividual rdf:about="http://purl.obolibrary.org/obo/GAZ_00030448">
        <obo:RO_0001025 rdf:resource="http://purl.obolibrary.org/obo/GAZ_00010359"/>
        <oboInOwl:hasOBONamespace>GAZ</oboInOwl:hasOBONamespace>
        <oboInOwl:id>GAZ:00030448</oboInOwl:id>
        <rdfs:label>Abu Ghraib District</rdfs:label>
    </owl:NamedIndividual>
    


    <!-- http://purl.obolibrary.org/obo/GAZ_00030449 -->

    <owl:NamedIndividual rdf:about="http://purl.obolibrary.org/obo/GAZ_00030449">
        <rdf:type rdf:resource="http://purl.obolibrary.org/obo/ENVO_00000004"/>
        <obo:RO_0001025 rdf:resource="http://purl.obolibrary.org/obo/GAZ_02000627"/>
        <obo:IAO_0000115>A district in Al Anbar Governorate, Iraq. It is centred around the city of Ramadi.</obo:IAO_0000115>
        <oboInOwl:hasOBONamespace>GAZ</oboInOwl:hasOBONamespace>
        <oboInOwl:id>GAZ:00030449</oboInOwl:id>
        <rdfs:label>Ramadi District</rdfs:label>
    </owl:NamedIndividual>
    


    <!-- http://purl.obolibrary.org/obo/GAZ_00030450 -->

    <owl:NamedIndividual rdf:about="http://purl.obolibrary.org/obo/GAZ_00030450">
        <rdf:type rdf:resource="http://purl.obolibrary.org/obo/ENVO_00000004"/>
        <obo:RO_0001025 rdf:resource="http://purl.obolibrary.org/obo/GAZ_02000627"/>
        <obo:IAO_0000115>A district in Al Anbar Governorate, Iraq. It is centred around the city of Hit.</obo:IAO_0000115>
        <oboInOwl:hasOBONamespace>GAZ</oboInOwl:hasOBONamespace>
        <oboInOwl:id>GAZ:00030450</oboInOwl:id>
        <rdfs:label>Heet District</rdfs:label>
    </owl:NamedIndividual>
    


    <!-- http://purl.obolibrary.org/obo/GAZ_00030451 -->

    <owl:NamedIndividual rdf:about="http://purl.obolibrary.org/obo/GAZ_00030451">
        <rdf:type rdf:resource="http://purl.obolibrary.org/obo/ENVO_00000004"/>
        <obo:RO_0001025 rdf:resource="http://purl.obolibrary.org/obo/GAZ_02000627"/>
        <obo:IAO_0000115>A district in Al Anbar Governorate, Iraq. It is centred around the town of Anah.</obo:IAO_0000115>
        <oboInOwl:hasOBONamespace>GAZ</oboInOwl:hasOBONamespace>
        <oboInOwl:id>GAZ:00030451</oboInOwl:id>
        <rdfs:label>Ana District</rdfs:label>
    </owl:NamedIndividual>
    


    <!-- http://purl.obolibrary.org/obo/GAZ_00030452 -->

    <owl:NamedIndividual rdf:about="http://purl.obolibrary.org/obo/GAZ_00030452">
        <rdf:type rdf:resource="http://purl.obolibrary.org/obo/ENVO_00000004"/>
        <obo:RO_0001025 rdf:resource="http://purl.obolibrary.org/obo/GAZ_02000627"/>
        <obo:IAO_0000115>A district in Al Anbar Governorate, Iraq. It is centred around the town of Ar Rutba.</obo:IAO_0000115>
        <oboInOwl:hasOBONamespace>GAZ</oboInOwl:hasOBONamespace>
        <oboInOwl:id>GAZ:00030452</oboInOwl:id>
        <rdfs:label>Al-Rutba District</rdfs:label>
    </owl:NamedIndividual>
    


    <!-- http://purl.obolibrary.org/obo/GAZ_00030453 -->

    <owl:NamedIndividual rdf:about="http://purl.obolibrary.org/obo/GAZ_00030453">
        <rdf:type rdf:resource="http://purl.obolibrary.org/obo/ENVO_00000004"/>
        <obo:RO_0001025 rdf:resource="http://purl.obolibrary.org/obo/GAZ_02000627"/>
        <obo:IAO_0000115>A district in Al Anbar Governorate, Iraq. It is centred around the city of Haditha.</obo:IAO_0000115>
        <oboInOwl:hasOBONamespace>GAZ</oboInOwl:hasOBONamespace>
        <oboInOwl:id>GAZ:00030453</oboInOwl:id>
        <rdfs:label>Haditha District</rdfs:label>
    </owl:NamedIndividual>
    


    <!-- http://purl.obolibrary.org/obo/GAZ_00030454 -->

    <owl:NamedIndividual rdf:about="http://purl.obolibrary.org/obo/GAZ_00030454">
        <rdf:type rdf:resource="http://purl.obolibrary.org/obo/ENVO_00000004"/>
        <obo:RO_0001025 rdf:resource="http://purl.obolibrary.org/obo/GAZ_02000627"/>
        <obo:IAO_0000115>A district in Al Anbar Governorate, Iraq. It is centred around the town of Al-Qa&apos;im.</obo:IAO_0000115>
        <oboInOwl:hasOBONamespace>GAZ</oboInOwl:hasOBONamespace>
        <oboInOwl:id>GAZ:00030454</oboInOwl:id>
        <rdfs:label>Al-Ka&apos;im District</rdfs:label>
    </owl:NamedIndividual>
    


    <!-- http://purl.obolibrary.org/obo/GAZ_00030455 -->

    <owl:NamedIndividual rdf:about="http://purl.obolibrary.org/obo/GAZ_00030455">
        <obo:RO_0001025 rdf:resource="http://purl.obolibrary.org/obo/GAZ_02000622"/>
        <oboInOwl:hasOBONamespace>GAZ</oboInOwl:hasOBONamespace>
        <oboInOwl:id>GAZ:00030455</oboInOwl:id>
        <rdfs:label>Mahmudiya District</rdfs:label>
    </owl:NamedIndividual>
    


    <!-- http://purl.obolibrary.org/obo/GAZ_00030456 -->

    <owl:NamedIndividual rdf:about="http://purl.obolibrary.org/obo/GAZ_00030456">
        <obo:RO_0001025 rdf:resource="http://purl.obolibrary.org/obo/GAZ_02000622"/>
        <oboInOwl:hasOBONamespace>GAZ</oboInOwl:hasOBONamespace>
        <oboInOwl:id>GAZ:00030456</oboInOwl:id>
        <rdfs:label>Hashimiya District</rdfs:label>
    </owl:NamedIndividual>
    


    <!-- http://purl.obolibrary.org/obo/GAZ_00030457 -->

    <owl:NamedIndividual rdf:about="http://purl.obolibrary.org/obo/GAZ_00030457">
        <obo:RO_0001025 rdf:resource="http://purl.obolibrary.org/obo/GAZ_02000622"/>
        <oboInOwl:hasOBONamespace>GAZ</oboInOwl:hasOBONamespace>
        <oboInOwl:id>GAZ:00030457</oboInOwl:id>
        <rdfs:label>Al-Mada&apos;in District</rdfs:label>
    </owl:NamedIndividual>
    


    <!-- http://purl.obolibrary.org/obo/GAZ_00030458 -->

    <owl:NamedIndividual rdf:about="http://purl.obolibrary.org/obo/GAZ_00030458">
        <obo:RO_0001025 rdf:resource="http://purl.obolibrary.org/obo/GAZ_02000622"/>
        <oboInOwl:hasOBONamespace>GAZ</oboInOwl:hasOBONamespace>
        <oboInOwl:id>GAZ:00030458</oboInOwl:id>
        <rdfs:label>Al-Musayab District</rdfs:label>
    </owl:NamedIndividual>
    


    <!-- http://purl.obolibrary.org/obo/GAZ_00030459 -->

    <owl:NamedIndividual rdf:about="http://purl.obolibrary.org/obo/GAZ_00030459">
        <obo:RO_0001025 rdf:resource="http://purl.obolibrary.org/obo/GAZ_02000622"/>
        <oboInOwl:hasOBONamespace>GAZ</oboInOwl:hasOBONamespace>
        <oboInOwl:id>GAZ:00030459</oboInOwl:id>
        <rdfs:label>Hilla District</rdfs:label>
    </owl:NamedIndividual>
    


    <!-- http://purl.obolibrary.org/obo/GAZ_00030460 -->

    <owl:NamedIndividual rdf:about="http://purl.obolibrary.org/obo/GAZ_00030460">
        <obo:RO_0001025 rdf:resource="http://purl.obolibrary.org/obo/GAZ_02000622"/>
        <oboInOwl:hasOBONamespace>GAZ</oboInOwl:hasOBONamespace>
        <oboInOwl:id>GAZ:00030460</oboInOwl:id>
        <rdfs:label>Al-Mahawil District</rdfs:label>
    </owl:NamedIndividual>
    


    <!-- http://purl.obolibrary.org/obo/GAZ_00030461 -->

    <owl:NamedIndividual rdf:about="http://purl.obolibrary.org/obo/GAZ_00030461">
        <obo:RO_0001025 rdf:resource="http://purl.obolibrary.org/obo/GAZ_00250964"/>
        <oboInOwl:hasOBONamespace>GAZ</oboInOwl:hasOBONamespace>
        <oboInOwl:id>GAZ:00030461</oboInOwl:id>
        <rdfs:label>Adhamiya District</rdfs:label>
    </owl:NamedIndividual>
    


    <!-- http://purl.obolibrary.org/obo/GAZ_00030462 -->

    <owl:NamedIndividual rdf:about="http://purl.obolibrary.org/obo/GAZ_00030462">
        <obo:RO_0001025 rdf:resource="http://purl.obolibrary.org/obo/GAZ_02000625"/>
        <oboInOwl:hasOBONamespace>GAZ</oboInOwl:hasOBONamespace>
        <oboInOwl:id>GAZ:00030462</oboInOwl:id>
        <rdfs:label>Sumel District</rdfs:label>
    </owl:NamedIndividual>
    


    <!-- http://purl.obolibrary.org/obo/GAZ_00030463 -->

    <owl:NamedIndividual rdf:about="http://purl.obolibrary.org/obo/GAZ_00030463">
        <obo:RO_0001025 rdf:resource="http://purl.obolibrary.org/obo/GAZ_02000625"/>
        <oboInOwl:hasOBONamespace>GAZ</oboInOwl:hasOBONamespace>
        <oboInOwl:id>GAZ:00030463</oboInOwl:id>
        <rdfs:label>Zakho District</rdfs:label>
    </owl:NamedIndividual>
    


    <!-- http://purl.obolibrary.org/obo/GAZ_00030464 -->

    <owl:NamedIndividual rdf:about="http://purl.obolibrary.org/obo/GAZ_00030464">
        <obo:RO_0001025 rdf:resource="http://purl.obolibrary.org/obo/GAZ_02000625"/>
        <oboInOwl:hasOBONamespace>GAZ</oboInOwl:hasOBONamespace>
        <oboInOwl:id>GAZ:00030464</oboInOwl:id>
        <rdfs:label>Amedi District</rdfs:label>
    </owl:NamedIndividual>
    


    <!-- http://purl.obolibrary.org/obo/GAZ_00030465 -->

    <owl:NamedIndividual rdf:about="http://purl.obolibrary.org/obo/GAZ_00030465">
        <obo:RO_0001025 rdf:resource="http://purl.obolibrary.org/obo/GAZ_02000625"/>
        <oboInOwl:hasOBONamespace>GAZ</oboInOwl:hasOBONamespace>
        <oboInOwl:id>GAZ:00030465</oboInOwl:id>
        <rdfs:label>Dahuk District</rdfs:label>
    </owl:NamedIndividual>
    


    <!-- http://purl.obolibrary.org/obo/GAZ_00030466 -->

    <owl:NamedIndividual rdf:about="http://purl.obolibrary.org/obo/GAZ_00030466">
        <obo:RO_0001025 rdf:resource="http://purl.obolibrary.org/obo/GAZ_02000620"/>
        <oboInOwl:hasOBONamespace>GAZ</oboInOwl:hasOBONamespace>
        <oboInOwl:id>GAZ:00030466</oboInOwl:id>
        <rdfs:label>Khanaqin District</rdfs:label>
    </owl:NamedIndividual>
    


    <!-- http://purl.obolibrary.org/obo/GAZ_00030467 -->

    <owl:NamedIndividual rdf:about="http://purl.obolibrary.org/obo/GAZ_00030467">
        <obo:RO_0001025 rdf:resource="http://purl.obolibrary.org/obo/GAZ_02000620"/>
        <oboInOwl:hasOBONamespace>GAZ</oboInOwl:hasOBONamespace>
        <oboInOwl:id>GAZ:00030467</oboInOwl:id>
        <rdfs:label>Kifri District</rdfs:label>
    </owl:NamedIndividual>
    


    <!-- http://purl.obolibrary.org/obo/GAZ_00030468 -->

    <owl:NamedIndividual rdf:about="http://purl.obolibrary.org/obo/GAZ_00030468">
        <obo:RO_0001025 rdf:resource="http://purl.obolibrary.org/obo/GAZ_02000620"/>
        <oboInOwl:hasOBONamespace>GAZ</oboInOwl:hasOBONamespace>
        <oboInOwl:id>GAZ:00030468</oboInOwl:id>
        <rdfs:label>Al-Khalis District</rdfs:label>
    </owl:NamedIndividual>
    


    <!-- http://purl.obolibrary.org/obo/GAZ_00030469 -->

    <owl:NamedIndividual rdf:about="http://purl.obolibrary.org/obo/GAZ_00030469">
        <obo:RO_0001025 rdf:resource="http://purl.obolibrary.org/obo/GAZ_02000620"/>
        <oboInOwl:hasOBONamespace>GAZ</oboInOwl:hasOBONamespace>
        <oboInOwl:id>GAZ:00030469</oboInOwl:id>
        <rdfs:label>Al-Muqdadiya District</rdfs:label>
    </owl:NamedIndividual>
    


    <!-- http://purl.obolibrary.org/obo/GAZ_00030470 -->

    <owl:NamedIndividual rdf:about="http://purl.obolibrary.org/obo/GAZ_00030470">
        <obo:RO_0001025 rdf:resource="http://purl.obolibrary.org/obo/GAZ_02000620"/>
        <oboInOwl:hasOBONamespace>GAZ</oboInOwl:hasOBONamespace>
        <oboInOwl:id>GAZ:00030470</oboInOwl:id>
        <rdfs:label>Baladrooz District</rdfs:label>
    </owl:NamedIndividual>
    


    <!-- http://purl.obolibrary.org/obo/GAZ_00030471 -->

    <owl:NamedIndividual rdf:about="http://purl.obolibrary.org/obo/GAZ_00030471">
        <obo:RO_0001025 rdf:resource="http://purl.obolibrary.org/obo/GAZ_02000620"/>
        <oboInOwl:hasOBONamespace>GAZ</oboInOwl:hasOBONamespace>
        <oboInOwl:id>GAZ:00030471</oboInOwl:id>
        <rdfs:label>Ba&apos;quba District</rdfs:label>
    </owl:NamedIndividual>
    


    <!-- http://purl.obolibrary.org/obo/GAZ_00030472 -->

    <owl:NamedIndividual rdf:about="http://purl.obolibrary.org/obo/GAZ_00030472">
        <obo:RO_0001025 rdf:resource="http://purl.obolibrary.org/obo/GAZ_02000614"/>
        <oboInOwl:hasOBONamespace>GAZ</oboInOwl:hasOBONamespace>
        <oboInOwl:id>GAZ:00030472</oboInOwl:id>
        <rdfs:label>Karbala District</rdfs:label>
    </owl:NamedIndividual>
    


    <!-- http://purl.obolibrary.org/obo/GAZ_00030473 -->

    <owl:NamedIndividual rdf:about="http://purl.obolibrary.org/obo/GAZ_00030473">
        <obo:RO_0001025 rdf:resource="http://purl.obolibrary.org/obo/GAZ_02000614"/>
        <oboInOwl:hasOBONamespace>GAZ</oboInOwl:hasOBONamespace>
        <oboInOwl:id>GAZ:00030473</oboInOwl:id>
        <rdfs:label>Al-Hindiya District</rdfs:label>
    </owl:NamedIndividual>
    


    <!-- http://purl.obolibrary.org/obo/GAZ_00030474 -->

    <owl:NamedIndividual rdf:about="http://purl.obolibrary.org/obo/GAZ_00030474">
        <obo:RO_0001025 rdf:resource="http://purl.obolibrary.org/obo/GAZ_02000614"/>
        <oboInOwl:hasOBONamespace>GAZ</oboInOwl:hasOBONamespace>
        <oboInOwl:id>GAZ:00030474</oboInOwl:id>
        <rdfs:label>Ain Al-Tamur District</rdfs:label>
    </owl:NamedIndividual>
    


    <!-- http://purl.obolibrary.org/obo/GAZ_00030475 -->

    <owl:NamedIndividual rdf:about="http://purl.obolibrary.org/obo/GAZ_00030475">
        <obo:RO_0001025 rdf:resource="http://purl.obolibrary.org/obo/GAZ_02000619"/>
        <oboInOwl:hasOBONamespace>GAZ</oboInOwl:hasOBONamespace>
        <oboInOwl:id>GAZ:00030475</oboInOwl:id>
        <rdfs:label>Al-Salman District</rdfs:label>
    </owl:NamedIndividual>
    


    <!-- http://purl.obolibrary.org/obo/GAZ_00030476 -->

    <owl:NamedIndividual rdf:about="http://purl.obolibrary.org/obo/GAZ_00030476">
        <obo:RO_0001025 rdf:resource="http://purl.obolibrary.org/obo/GAZ_02000619"/>
        <oboInOwl:hasOBONamespace>GAZ</oboInOwl:hasOBONamespace>
        <oboInOwl:id>GAZ:00030476</oboInOwl:id>
        <rdfs:label>Al-Rumaitha District</rdfs:label>
    </owl:NamedIndividual>
    


    <!-- http://purl.obolibrary.org/obo/GAZ_00030477 -->

    <owl:NamedIndividual rdf:about="http://purl.obolibrary.org/obo/GAZ_00030477">
        <obo:RO_0001025 rdf:resource="http://purl.obolibrary.org/obo/GAZ_02000619"/>
        <oboInOwl:hasOBONamespace>GAZ</oboInOwl:hasOBONamespace>
        <oboInOwl:id>GAZ:00030477</oboInOwl:id>
        <rdfs:label>Al-Khidhir District</rdfs:label>
    </owl:NamedIndividual>
    


    <!-- http://purl.obolibrary.org/obo/GAZ_00030478 -->

    <owl:NamedIndividual rdf:about="http://purl.obolibrary.org/obo/GAZ_00030478">
        <obo:RO_0001025 rdf:resource="http://purl.obolibrary.org/obo/GAZ_02000619"/>
        <oboInOwl:hasOBONamespace>GAZ</oboInOwl:hasOBONamespace>
        <oboInOwl:id>GAZ:00030478</oboInOwl:id>
        <rdfs:label>Al-Samawa District</rdfs:label>
    </owl:NamedIndividual>
    


    <!-- http://purl.obolibrary.org/obo/GAZ_00030479 -->

    <owl:NamedIndividual rdf:about="http://purl.obolibrary.org/obo/GAZ_00030479">
        <obo:RO_0001025 rdf:resource="http://purl.obolibrary.org/obo/GAZ_02000618"/>
        <oboInOwl:hasOBONamespace>GAZ</oboInOwl:hasOBONamespace>
        <oboInOwl:id>GAZ:00030479</oboInOwl:id>
        <rdfs:label>Najaf District</rdfs:label>
    </owl:NamedIndividual>
    


    <!-- http://purl.obolibrary.org/obo/GAZ_00030480 -->

    <owl:NamedIndividual rdf:about="http://purl.obolibrary.org/obo/GAZ_00030480">
        <obo:RO_0001025 rdf:resource="http://purl.obolibrary.org/obo/GAZ_02000618"/>
        <oboInOwl:hasOBONamespace>GAZ</oboInOwl:hasOBONamespace>
        <oboInOwl:id>GAZ:00030480</oboInOwl:id>
        <rdfs:label>Kufa District</rdfs:label>
    </owl:NamedIndividual>
    


    <!-- http://purl.obolibrary.org/obo/GAZ_00030481 -->

    <owl:NamedIndividual rdf:about="http://purl.obolibrary.org/obo/GAZ_00030481">
        <obo:RO_0001025 rdf:resource="http://purl.obolibrary.org/obo/GAZ_02000618"/>
        <oboInOwl:hasOBONamespace>GAZ</oboInOwl:hasOBONamespace>
        <oboInOwl:id>GAZ:00030481</oboInOwl:id>
        <rdfs:label>Al-Manathera District</rdfs:label>
    </owl:NamedIndividual>
    


    <!-- http://purl.obolibrary.org/obo/GAZ_00030482 -->

    <owl:NamedIndividual rdf:about="http://purl.obolibrary.org/obo/GAZ_00030482">
        <obo:RO_0001025 rdf:resource="http://purl.obolibrary.org/obo/GAZ_02000616"/>
        <oboInOwl:hasOBONamespace>GAZ</oboInOwl:hasOBONamespace>
        <oboInOwl:id>GAZ:00030482</oboInOwl:id>
        <rdfs:label>Al-Shirqat District</rdfs:label>
    </owl:NamedIndividual>
    


    <!-- http://purl.obolibrary.org/obo/GAZ_00030483 -->

    <owl:NamedIndividual rdf:about="http://purl.obolibrary.org/obo/GAZ_00030483">
        <obo:RO_0001025 rdf:resource="http://purl.obolibrary.org/obo/GAZ_02000616"/>
        <oboInOwl:hasOBONamespace>GAZ</oboInOwl:hasOBONamespace>
        <oboInOwl:id>GAZ:00030483</oboInOwl:id>
        <rdfs:label>Balad District</rdfs:label>
    </owl:NamedIndividual>
    


    <!-- http://purl.obolibrary.org/obo/GAZ_00030484 -->

    <owl:NamedIndividual rdf:about="http://purl.obolibrary.org/obo/GAZ_00030484">
        <obo:RO_0001025 rdf:resource="http://purl.obolibrary.org/obo/GAZ_02000616"/>
        <oboInOwl:hasOBONamespace>GAZ</oboInOwl:hasOBONamespace>
        <oboInOwl:id>GAZ:00030484</oboInOwl:id>
        <rdfs:label>Al-Daur District</rdfs:label>
    </owl:NamedIndividual>
    


    <!-- http://purl.obolibrary.org/obo/GAZ_00030485 -->

    <owl:NamedIndividual rdf:about="http://purl.obolibrary.org/obo/GAZ_00030485">
        <obo:RO_0001025 rdf:resource="http://purl.obolibrary.org/obo/GAZ_02000616"/>
        <oboInOwl:hasOBONamespace>GAZ</oboInOwl:hasOBONamespace>
        <oboInOwl:id>GAZ:00030485</oboInOwl:id>
        <rdfs:label>Al-Faris District</rdfs:label>
    </owl:NamedIndividual>
    


    <!-- http://purl.obolibrary.org/obo/GAZ_00030486 -->

    <owl:NamedIndividual rdf:about="http://purl.obolibrary.org/obo/GAZ_00030486">
        <obo:RO_0001025 rdf:resource="http://purl.obolibrary.org/obo/GAZ_02000616"/>
        <oboInOwl:hasOBONamespace>GAZ</oboInOwl:hasOBONamespace>
        <oboInOwl:id>GAZ:00030486</oboInOwl:id>
        <rdfs:label>Samarra District</rdfs:label>
    </owl:NamedIndividual>
    


    <!-- http://purl.obolibrary.org/obo/GAZ_00030487 -->

    <owl:NamedIndividual rdf:about="http://purl.obolibrary.org/obo/GAZ_00030487">
        <obo:RO_0001025 rdf:resource="http://purl.obolibrary.org/obo/GAZ_02000616"/>
        <oboInOwl:hasOBONamespace>GAZ</oboInOwl:hasOBONamespace>
        <oboInOwl:id>GAZ:00030487</oboInOwl:id>
        <rdfs:label>Tooz District</rdfs:label>
    </owl:NamedIndividual>
    


    <!-- http://purl.obolibrary.org/obo/GAZ_00030488 -->

    <owl:NamedIndividual rdf:about="http://purl.obolibrary.org/obo/GAZ_00030488">
        <obo:RO_0001025 rdf:resource="http://purl.obolibrary.org/obo/GAZ_02000616"/>
        <oboInOwl:hasOBONamespace>GAZ</oboInOwl:hasOBONamespace>
        <oboInOwl:id>GAZ:00030488</oboInOwl:id>
        <rdfs:label>Tikrit District</rdfs:label>
    </owl:NamedIndividual>
    


    <!-- http://purl.obolibrary.org/obo/GAZ_00030489 -->

    <owl:NamedIndividual rdf:about="http://purl.obolibrary.org/obo/GAZ_00030489">
        <obo:RO_0001025 rdf:resource="http://purl.obolibrary.org/obo/GAZ_02000616"/>
        <oboInOwl:hasOBONamespace>GAZ</oboInOwl:hasOBONamespace>
        <oboInOwl:id>GAZ:00030489</oboInOwl:id>
        <rdfs:label>Baiji District</rdfs:label>
    </owl:NamedIndividual>
    


    <!-- http://purl.obolibrary.org/obo/GAZ_00030490 -->

    <owl:NamedIndividual rdf:about="http://purl.obolibrary.org/obo/GAZ_00030490">
        <obo:RO_0001025 rdf:resource="http://purl.obolibrary.org/obo/GAZ_02000615"/>
        <oboInOwl:hasOBONamespace>GAZ</oboInOwl:hasOBONamespace>
        <oboInOwl:id>GAZ:00030490</oboInOwl:id>
        <rdfs:label>Penjwin District</rdfs:label>
    </owl:NamedIndividual>
    


    <!-- http://purl.obolibrary.org/obo/GAZ_00030491 -->

    <owl:NamedIndividual rdf:about="http://purl.obolibrary.org/obo/GAZ_00030491">
        <obo:RO_0001025 rdf:resource="http://purl.obolibrary.org/obo/GAZ_02000615"/>
        <oboInOwl:hasOBONamespace>GAZ</oboInOwl:hasOBONamespace>
        <oboInOwl:id>GAZ:00030491</oboInOwl:id>
        <rdfs:label>Rania District</rdfs:label>
    </owl:NamedIndividual>
    


    <!-- http://purl.obolibrary.org/obo/GAZ_00030492 -->

    <owl:NamedIndividual rdf:about="http://purl.obolibrary.org/obo/GAZ_00030492">
        <obo:RO_0001025 rdf:resource="http://purl.obolibrary.org/obo/GAZ_02000615"/>
        <oboInOwl:hasOBONamespace>GAZ</oboInOwl:hasOBONamespace>
        <oboInOwl:id>GAZ:00030492</oboInOwl:id>
        <rdfs:label>Chamchamal District</rdfs:label>
    </owl:NamedIndividual>
    


    <!-- http://purl.obolibrary.org/obo/GAZ_00030493 -->

    <owl:NamedIndividual rdf:about="http://purl.obolibrary.org/obo/GAZ_00030493">
        <obo:RO_0001025 rdf:resource="http://purl.obolibrary.org/obo/GAZ_02000615"/>
        <oboInOwl:hasOBONamespace>GAZ</oboInOwl:hasOBONamespace>
        <oboInOwl:id>GAZ:00030493</oboInOwl:id>
        <rdfs:label>Halabja District</rdfs:label>
    </owl:NamedIndividual>
    


    <!-- http://purl.obolibrary.org/obo/GAZ_00030494 -->

    <owl:NamedIndividual rdf:about="http://purl.obolibrary.org/obo/GAZ_00030494">
        <obo:RO_0001025 rdf:resource="http://purl.obolibrary.org/obo/GAZ_02000615"/>
        <oboInOwl:hasOBONamespace>GAZ</oboInOwl:hasOBONamespace>
        <oboInOwl:id>GAZ:00030494</oboInOwl:id>
        <rdfs:label>Sulaymaniya District</rdfs:label>
    </owl:NamedIndividual>
    


    <!-- http://purl.obolibrary.org/obo/GAZ_00030495 -->

    <owl:NamedIndividual rdf:about="http://purl.obolibrary.org/obo/GAZ_00030495">
        <obo:RO_0001025 rdf:resource="http://purl.obolibrary.org/obo/GAZ_02000615"/>
        <oboInOwl:hasOBONamespace>GAZ</oboInOwl:hasOBONamespace>
        <oboInOwl:id>GAZ:00030495</oboInOwl:id>
        <rdfs:label>Dokan District</rdfs:label>
    </owl:NamedIndividual>
    


    <!-- http://purl.obolibrary.org/obo/GAZ_00030496 -->

    <owl:NamedIndividual rdf:about="http://purl.obolibrary.org/obo/GAZ_00030496">
        <obo:RO_0001025 rdf:resource="http://purl.obolibrary.org/obo/GAZ_02000615"/>
        <oboInOwl:hasOBONamespace>GAZ</oboInOwl:hasOBONamespace>
        <oboInOwl:id>GAZ:00030496</oboInOwl:id>
        <rdfs:label>Pshdar District</rdfs:label>
    </owl:NamedIndividual>
    


    <!-- http://purl.obolibrary.org/obo/GAZ_00030497 -->

    <owl:NamedIndividual rdf:about="http://purl.obolibrary.org/obo/GAZ_00030497">
        <obo:RO_0001025 rdf:resource="http://purl.obolibrary.org/obo/GAZ_02000615"/>
        <oboInOwl:hasOBONamespace>GAZ</oboInOwl:hasOBONamespace>
        <oboInOwl:id>GAZ:00030497</oboInOwl:id>
        <rdfs:label>Sharbazher District</rdfs:label>
    </owl:NamedIndividual>
    


    <!-- http://purl.obolibrary.org/obo/GAZ_00030498 -->

    <owl:NamedIndividual rdf:about="http://purl.obolibrary.org/obo/GAZ_00030498">
        <obo:RO_0001025 rdf:resource="http://purl.obolibrary.org/obo/GAZ_02000615"/>
        <oboInOwl:hasOBONamespace>GAZ</oboInOwl:hasOBONamespace>
        <oboInOwl:id>GAZ:00030498</oboInOwl:id>
        <rdfs:label>Kalar District</rdfs:label>
    </owl:NamedIndividual>
    


    <!-- http://purl.obolibrary.org/obo/GAZ_00030499 -->

    <owl:NamedIndividual rdf:about="http://purl.obolibrary.org/obo/GAZ_00030499">
        <obo:RO_0001025 rdf:resource="http://purl.obolibrary.org/obo/GAZ_02000615"/>
        <oboInOwl:hasOBONamespace>GAZ</oboInOwl:hasOBONamespace>
        <oboInOwl:id>GAZ:00030499</oboInOwl:id>
        <rdfs:label>Darbandokeh District</rdfs:label>
    </owl:NamedIndividual>
    


    <!-- http://purl.obolibrary.org/obo/GAZ_00030500 -->

    <owl:NamedIndividual rdf:about="http://purl.obolibrary.org/obo/GAZ_00030500">
        <obo:RO_0001025 rdf:resource="http://purl.obolibrary.org/obo/GAZ_02000613"/>
        <oboInOwl:hasOBONamespace>GAZ</oboInOwl:hasOBONamespace>
        <oboInOwl:id>GAZ:00030500</oboInOwl:id>
        <rdfs:label>Al-Suwaira District</rdfs:label>
    </owl:NamedIndividual>
    


    <!-- http://purl.obolibrary.org/obo/GAZ_00030501 -->

    <owl:NamedIndividual rdf:about="http://purl.obolibrary.org/obo/GAZ_00030501">
        <obo:RO_0001025 rdf:resource="http://purl.obolibrary.org/obo/GAZ_02000613"/>
        <oboInOwl:hasOBONamespace>GAZ</oboInOwl:hasOBONamespace>
        <oboInOwl:id>GAZ:00030501</oboInOwl:id>
        <rdfs:label>Al-Na&apos;maniya District</rdfs:label>
    </owl:NamedIndividual>
    


    <!-- http://purl.obolibrary.org/obo/GAZ_00030502 -->

    <owl:NamedIndividual rdf:about="http://purl.obolibrary.org/obo/GAZ_00030502">
        <obo:RO_0001025 rdf:resource="http://purl.obolibrary.org/obo/GAZ_02000613"/>
        <oboInOwl:hasOBONamespace>GAZ</oboInOwl:hasOBONamespace>
        <oboInOwl:id>GAZ:00030502</oboInOwl:id>
        <rdfs:label>Badra District</rdfs:label>
    </owl:NamedIndividual>
    


    <!-- http://purl.obolibrary.org/obo/GAZ_00030503 -->

    <owl:NamedIndividual rdf:about="http://purl.obolibrary.org/obo/GAZ_00030503">
        <obo:RO_0001025 rdf:resource="http://purl.obolibrary.org/obo/GAZ_02000613"/>
        <oboInOwl:hasOBONamespace>GAZ</oboInOwl:hasOBONamespace>
        <oboInOwl:id>GAZ:00030503</oboInOwl:id>
        <rdfs:label>Al-Hai District</rdfs:label>
    </owl:NamedIndividual>
    


    <!-- http://purl.obolibrary.org/obo/GAZ_00030504 -->

    <owl:NamedIndividual rdf:about="http://purl.obolibrary.org/obo/GAZ_00030504">
        <obo:RO_0001025 rdf:resource="http://purl.obolibrary.org/obo/GAZ_02000613"/>
        <oboInOwl:hasOBONamespace>GAZ</oboInOwl:hasOBONamespace>
        <oboInOwl:id>GAZ:00030504</oboInOwl:id>
        <rdfs:label>Kut District</rdfs:label>
    </owl:NamedIndividual>
    


    <!-- http://purl.obolibrary.org/obo/GAZ_00030505 -->

    <owl:NamedIndividual rdf:about="http://purl.obolibrary.org/obo/GAZ_00030505">
        <obo:RO_0001025 rdf:resource="http://purl.obolibrary.org/obo/GAZ_02000626"/>
        <oboInOwl:hasOBONamespace>GAZ</oboInOwl:hasOBONamespace>
        <oboInOwl:id>GAZ:00030505</oboInOwl:id>
        <rdfs:label>Suq Al-Shoyokh District</rdfs:label>
    </owl:NamedIndividual>
    


    <!-- http://purl.obolibrary.org/obo/GAZ_00030506 -->

    <owl:NamedIndividual rdf:about="http://purl.obolibrary.org/obo/GAZ_00030506">
        <obo:RO_0001025 rdf:resource="http://purl.obolibrary.org/obo/GAZ_02000626"/>
        <oboInOwl:hasOBONamespace>GAZ</oboInOwl:hasOBONamespace>
        <oboInOwl:id>GAZ:00030506</oboInOwl:id>
        <rdfs:label>Al-Shatra District</rdfs:label>
    </owl:NamedIndividual>
    


    <!-- http://purl.obolibrary.org/obo/GAZ_00030507 -->

    <owl:NamedIndividual rdf:about="http://purl.obolibrary.org/obo/GAZ_00030507">
        <obo:RO_0001025 rdf:resource="http://purl.obolibrary.org/obo/GAZ_02000626"/>
        <oboInOwl:hasOBONamespace>GAZ</oboInOwl:hasOBONamespace>
        <oboInOwl:id>GAZ:00030507</oboInOwl:id>
        <rdfs:label>Al-Chibayish District</rdfs:label>
    </owl:NamedIndividual>
    


    <!-- http://purl.obolibrary.org/obo/GAZ_00030508 -->

    <owl:NamedIndividual rdf:about="http://purl.obolibrary.org/obo/GAZ_00030508">
        <obo:RO_0001025 rdf:resource="http://purl.obolibrary.org/obo/GAZ_02000626"/>
        <oboInOwl:hasOBONamespace>GAZ</oboInOwl:hasOBONamespace>
        <oboInOwl:id>GAZ:00030508</oboInOwl:id>
        <rdfs:label>Al-Rifa&apos;i District</rdfs:label>
    </owl:NamedIndividual>
    


    <!-- http://purl.obolibrary.org/obo/GAZ_00030509 -->

    <owl:NamedIndividual rdf:about="http://purl.obolibrary.org/obo/GAZ_00030509">
        <obo:RO_0001025 rdf:resource="http://purl.obolibrary.org/obo/GAZ_02000626"/>
        <oboInOwl:hasOBONamespace>GAZ</oboInOwl:hasOBONamespace>
        <oboInOwl:id>GAZ:00030509</oboInOwl:id>
        <rdfs:label>Nassriya District</rdfs:label>
    </owl:NamedIndividual>
    


    <!-- http://purl.obolibrary.org/obo/GAZ_00030510 -->

    <owl:NamedIndividual rdf:about="http://purl.obolibrary.org/obo/GAZ_00030510">
        <obo:RO_0001025 rdf:resource="http://purl.obolibrary.org/obo/GAZ_02000623"/>
        <oboInOwl:hasOBONamespace>GAZ</oboInOwl:hasOBONamespace>
        <oboInOwl:id>GAZ:00030510</oboInOwl:id>
        <rdfs:label>Diwaniya District</rdfs:label>
    </owl:NamedIndividual>
    


    <!-- http://purl.obolibrary.org/obo/GAZ_00030511 -->

    <owl:NamedIndividual rdf:about="http://purl.obolibrary.org/obo/GAZ_00030511">
        <obo:RO_0001025 rdf:resource="http://purl.obolibrary.org/obo/GAZ_02000623"/>
        <oboInOwl:hasOBONamespace>GAZ</oboInOwl:hasOBONamespace>
        <oboInOwl:id>GAZ:00030511</oboInOwl:id>
        <rdfs:label>Al-Shamiya District</rdfs:label>
    </owl:NamedIndividual>
    


    <!-- http://purl.obolibrary.org/obo/GAZ_00030512 -->

    <owl:NamedIndividual rdf:about="http://purl.obolibrary.org/obo/GAZ_00030512">
        <obo:RO_0001025 rdf:resource="http://purl.obolibrary.org/obo/GAZ_02000623"/>
        <oboInOwl:hasOBONamespace>GAZ</oboInOwl:hasOBONamespace>
        <oboInOwl:id>GAZ:00030512</oboInOwl:id>
        <rdfs:label>Afaq District</rdfs:label>
    </owl:NamedIndividual>
    


    <!-- http://purl.obolibrary.org/obo/GAZ_00030513 -->

    <owl:NamedIndividual rdf:about="http://purl.obolibrary.org/obo/GAZ_00030513">
        <obo:RO_0001025 rdf:resource="http://purl.obolibrary.org/obo/GAZ_02000623"/>
        <oboInOwl:hasOBONamespace>GAZ</oboInOwl:hasOBONamespace>
        <oboInOwl:id>GAZ:00030513</oboInOwl:id>
        <rdfs:label>Hamza District</rdfs:label>
    </owl:NamedIndividual>
    


    <!-- http://purl.obolibrary.org/obo/GAZ_00030818 -->

    <owl:NamedIndividual rdf:about="http://purl.obolibrary.org/obo/GAZ_00030818">
        <obo:RO_0001025 rdf:resource="http://purl.obolibrary.org/obo/GAZ_02000617"/>
        <oboInOwl:hasOBONamespace>GAZ</oboInOwl:hasOBONamespace>
        <oboInOwl:id>GAZ:00030818</oboInOwl:id>
        <rdfs:label>Shaqlawa District</rdfs:label>
    </owl:NamedIndividual>
    


    <!-- http://purl.obolibrary.org/obo/GAZ_00030819 -->

    <owl:NamedIndividual rdf:about="http://purl.obolibrary.org/obo/GAZ_00030819">
        <obo:RO_0001025 rdf:resource="http://purl.obolibrary.org/obo/GAZ_02000617"/>
        <oboInOwl:hasOBONamespace>GAZ</oboInOwl:hasOBONamespace>
        <oboInOwl:id>GAZ:00030819</oboInOwl:id>
        <rdfs:label>Mergasur District</rdfs:label>
    </owl:NamedIndividual>
    


    <!-- http://purl.obolibrary.org/obo/GAZ_00030820 -->

    <owl:NamedIndividual rdf:about="http://purl.obolibrary.org/obo/GAZ_00030820">
        <obo:RO_0001025 rdf:resource="http://purl.obolibrary.org/obo/GAZ_02000617"/>
        <oboInOwl:hasOBONamespace>GAZ</oboInOwl:hasOBONamespace>
        <oboInOwl:id>GAZ:00030820</oboInOwl:id>
        <rdfs:label>Choman District</rdfs:label>
    </owl:NamedIndividual>
    


    <!-- http://purl.obolibrary.org/obo/GAZ_00030821 -->

    <owl:NamedIndividual rdf:about="http://purl.obolibrary.org/obo/GAZ_00030821">
        <obo:RO_0001025 rdf:resource="http://purl.obolibrary.org/obo/GAZ_02000617"/>
        <oboInOwl:hasOBONamespace>GAZ</oboInOwl:hasOBONamespace>
        <oboInOwl:id>GAZ:00030821</oboInOwl:id>
        <rdfs:label>Makhmur District</rdfs:label>
    </owl:NamedIndividual>
    


    <!-- http://purl.obolibrary.org/obo/GAZ_00030822 -->

    <owl:NamedIndividual rdf:about="http://purl.obolibrary.org/obo/GAZ_00030822">
        <obo:RO_0001025 rdf:resource="http://purl.obolibrary.org/obo/GAZ_02000617"/>
        <oboInOwl:hasOBONamespace>GAZ</oboInOwl:hasOBONamespace>
        <oboInOwl:id>GAZ:00030822</oboInOwl:id>
        <rdfs:label>Soran District</rdfs:label>
    </owl:NamedIndividual>
    


    <!-- http://purl.obolibrary.org/obo/GAZ_00030823 -->

    <owl:NamedIndividual rdf:about="http://purl.obolibrary.org/obo/GAZ_00030823">
        <obo:RO_0001025 rdf:resource="http://purl.obolibrary.org/obo/GAZ_02000617"/>
        <oboInOwl:hasOBONamespace>GAZ</oboInOwl:hasOBONamespace>
        <oboInOwl:id>GAZ:00030823</oboInOwl:id>
        <rdfs:label>Koisnjaq District</rdfs:label>
    </owl:NamedIndividual>
    


    <!-- http://purl.obolibrary.org/obo/GAZ_00030824 -->

    <owl:NamedIndividual rdf:about="http://purl.obolibrary.org/obo/GAZ_00030824">
        <obo:RO_0001025 rdf:resource="http://purl.obolibrary.org/obo/GAZ_02000617"/>
        <oboInOwl:hasOBONamespace>GAZ</oboInOwl:hasOBONamespace>
        <oboInOwl:id>GAZ:00030824</oboInOwl:id>
        <rdfs:label>Arbil District</rdfs:label>
    </owl:NamedIndividual>
    


    <!-- http://purl.obolibrary.org/obo/GAZ_00030825 -->

    <owl:NamedIndividual rdf:about="http://purl.obolibrary.org/obo/GAZ_00030825">
        <obo:RO_0001025 rdf:resource="http://purl.obolibrary.org/obo/GAZ_02000621"/>
        <oboInOwl:hasOBONamespace>GAZ</oboInOwl:hasOBONamespace>
        <oboInOwl:id>GAZ:00030825</oboInOwl:id>
        <rdfs:label>Kirkuk District</rdfs:label>
    </owl:NamedIndividual>
    


    <!-- http://purl.obolibrary.org/obo/GAZ_00030826 -->

    <owl:NamedIndividual rdf:about="http://purl.obolibrary.org/obo/GAZ_00030826">
        <obo:RO_0001025 rdf:resource="http://purl.obolibrary.org/obo/GAZ_02000621"/>
        <oboInOwl:hasOBONamespace>GAZ</oboInOwl:hasOBONamespace>
        <oboInOwl:id>GAZ:00030826</oboInOwl:id>
        <rdfs:label>Daquq District</rdfs:label>
    </owl:NamedIndividual>
    


    <!-- http://purl.obolibrary.org/obo/GAZ_00030827 -->

    <owl:NamedIndividual rdf:about="http://purl.obolibrary.org/obo/GAZ_00030827">
        <obo:RO_0001025 rdf:resource="http://purl.obolibrary.org/obo/GAZ_02000621"/>
        <oboInOwl:hasOBONamespace>GAZ</oboInOwl:hasOBONamespace>
        <oboInOwl:id>GAZ:00030827</oboInOwl:id>
        <rdfs:label>Al-Hawiga District</rdfs:label>
    </owl:NamedIndividual>
    


    <!-- http://purl.obolibrary.org/obo/GAZ_00030828 -->

    <owl:NamedIndividual rdf:about="http://purl.obolibrary.org/obo/GAZ_00030828">
        <obo:RO_0001025 rdf:resource="http://purl.obolibrary.org/obo/GAZ_02000621"/>
        <oboInOwl:hasOBONamespace>GAZ</oboInOwl:hasOBONamespace>
        <oboInOwl:id>GAZ:00030828</oboInOwl:id>
        <rdfs:label>Makhmur District</rdfs:label>
    </owl:NamedIndividual>
    


    <!-- http://purl.obolibrary.org/obo/GAZ_00030829 -->

    <owl:NamedIndividual rdf:about="http://purl.obolibrary.org/obo/GAZ_00030829">
        <obo:RO_0001025 rdf:resource="http://purl.obolibrary.org/obo/GAZ_02000624"/>
        <oboInOwl:hasOBONamespace>GAZ</oboInOwl:hasOBONamespace>
        <oboInOwl:id>GAZ:00030829</oboInOwl:id>
        <rdfs:label>Al-Mejar Al-Kabi District</rdfs:label>
    </owl:NamedIndividual>
    


    <!-- http://purl.obolibrary.org/obo/GAZ_00030830 -->

    <owl:NamedIndividual rdf:about="http://purl.obolibrary.org/obo/GAZ_00030830">
        <obo:RO_0001025 rdf:resource="http://purl.obolibrary.org/obo/GAZ_02000624"/>
        <oboInOwl:hasOBONamespace>GAZ</oboInOwl:hasOBONamespace>
        <oboInOwl:id>GAZ:00030830</oboInOwl:id>
        <rdfs:label>Qal&apos;at Saleh District</rdfs:label>
    </owl:NamedIndividual>
    


    <!-- http://purl.obolibrary.org/obo/GAZ_00030831 -->

    <owl:NamedIndividual rdf:about="http://purl.obolibrary.org/obo/GAZ_00030831">
        <obo:RO_0001025 rdf:resource="http://purl.obolibrary.org/obo/GAZ_02000624"/>
        <oboInOwl:hasOBONamespace>GAZ</oboInOwl:hasOBONamespace>
        <oboInOwl:id>GAZ:00030831</oboInOwl:id>
        <rdfs:label>Ali Al-Gharbi District</rdfs:label>
    </owl:NamedIndividual>
    


    <!-- http://purl.obolibrary.org/obo/GAZ_00030832 -->

    <owl:NamedIndividual rdf:about="http://purl.obolibrary.org/obo/GAZ_00030832">
        <obo:RO_0001025 rdf:resource="http://purl.obolibrary.org/obo/GAZ_02000624"/>
        <oboInOwl:hasOBONamespace>GAZ</oboInOwl:hasOBONamespace>
        <oboInOwl:id>GAZ:00030832</oboInOwl:id>
        <rdfs:label>Al-Kahla District</rdfs:label>
    </owl:NamedIndividual>
    


    <!-- http://purl.obolibrary.org/obo/GAZ_00030833 -->

    <owl:NamedIndividual rdf:about="http://purl.obolibrary.org/obo/GAZ_00030833">
        <obo:RO_0001025 rdf:resource="http://purl.obolibrary.org/obo/GAZ_02000624"/>
        <oboInOwl:hasOBONamespace>GAZ</oboInOwl:hasOBONamespace>
        <oboInOwl:id>GAZ:00030833</oboInOwl:id>
        <rdfs:label>Al-Maimouna District</rdfs:label>
    </owl:NamedIndividual>
    


    <!-- http://purl.obolibrary.org/obo/GAZ_00030834 -->

    <owl:NamedIndividual rdf:about="http://purl.obolibrary.org/obo/GAZ_00030834">
        <obo:RO_0001025 rdf:resource="http://purl.obolibrary.org/obo/GAZ_02000624"/>
        <oboInOwl:hasOBONamespace>GAZ</oboInOwl:hasOBONamespace>
        <oboInOwl:id>GAZ:00030834</oboInOwl:id>
        <rdfs:label>Amara District</rdfs:label>
    </owl:NamedIndividual>
    


    <!-- http://purl.obolibrary.org/obo/GAZ_00030835 -->

    <owl:NamedIndividual rdf:about="http://purl.obolibrary.org/obo/GAZ_00030835"/>
    


    <!-- http://purl.obolibrary.org/obo/GAZ_00030836 -->

    <owl:NamedIndividual rdf:about="http://purl.obolibrary.org/obo/GAZ_00030836">
        <obo:RO_0001025 rdf:resource="http://purl.obolibrary.org/obo/GAZ_00030835"/>
        <oboInOwl:hasOBONamespace>GAZ</oboInOwl:hasOBONamespace>
        <oboInOwl:id>GAZ:00030836</oboInOwl:id>
        <rdfs:label>Mosul District</rdfs:label>
    </owl:NamedIndividual>
    


    <!-- http://purl.obolibrary.org/obo/GAZ_00030837 -->

    <owl:NamedIndividual rdf:about="http://purl.obolibrary.org/obo/GAZ_00030837">
        <obo:RO_0001025 rdf:resource="http://purl.obolibrary.org/obo/GAZ_00030835"/>
        <oboInOwl:hasOBONamespace>GAZ</oboInOwl:hasOBONamespace>
        <oboInOwl:id>GAZ:00030837</oboInOwl:id>
        <rdfs:label>Tilkaif District</rdfs:label>
    </owl:NamedIndividual>
    


    <!-- http://purl.obolibrary.org/obo/GAZ_00030838 -->

    <owl:NamedIndividual rdf:about="http://purl.obolibrary.org/obo/GAZ_00030838">
        <obo:RO_0001025 rdf:resource="http://purl.obolibrary.org/obo/GAZ_00030835"/>
        <oboInOwl:hasOBONamespace>GAZ</oboInOwl:hasOBONamespace>
        <oboInOwl:id>GAZ:00030838</oboInOwl:id>
        <rdfs:label>Akre District</rdfs:label>
    </owl:NamedIndividual>
    


    <!-- http://purl.obolibrary.org/obo/GAZ_00030839 -->

    <owl:NamedIndividual rdf:about="http://purl.obolibrary.org/obo/GAZ_00030839">
        <obo:RO_0001025 rdf:resource="http://purl.obolibrary.org/obo/GAZ_00030835"/>
        <oboInOwl:hasOBONamespace>GAZ</oboInOwl:hasOBONamespace>
        <oboInOwl:id>GAZ:00030839</oboInOwl:id>
        <rdfs:label>Shekhan District</rdfs:label>
    </owl:NamedIndividual>
    


    <!-- http://purl.obolibrary.org/obo/GAZ_00030840 -->

    <owl:NamedIndividual rdf:about="http://purl.obolibrary.org/obo/GAZ_00030840">
        <obo:RO_0001025 rdf:resource="http://purl.obolibrary.org/obo/GAZ_00030835"/>
        <oboInOwl:hasOBONamespace>GAZ</oboInOwl:hasOBONamespace>
        <oboInOwl:id>GAZ:00030840</oboInOwl:id>
        <rdfs:label>Sinjar District</rdfs:label>
    </owl:NamedIndividual>
    


    <!-- http://purl.obolibrary.org/obo/GAZ_00030841 -->

    <owl:NamedIndividual rdf:about="http://purl.obolibrary.org/obo/GAZ_00030841">
        <obo:RO_0001025 rdf:resource="http://purl.obolibrary.org/obo/GAZ_00030835"/>
        <oboInOwl:hasOBONamespace>GAZ</oboInOwl:hasOBONamespace>
        <oboInOwl:id>GAZ:00030841</oboInOwl:id>
        <rdfs:label>Al-Ba&apos;aj District</rdfs:label>
    </owl:NamedIndividual>
    


    <!-- http://purl.obolibrary.org/obo/GAZ_00030842 -->

    <owl:NamedIndividual rdf:about="http://purl.obolibrary.org/obo/GAZ_00030842">
        <obo:RO_0001025 rdf:resource="http://purl.obolibrary.org/obo/GAZ_00030835"/>
        <oboInOwl:hasOBONamespace>GAZ</oboInOwl:hasOBONamespace>
        <oboInOwl:id>GAZ:00030842</oboInOwl:id>
        <rdfs:label>Al-Hamdaniya District</rdfs:label>
    </owl:NamedIndividual>
    


    <!-- http://purl.obolibrary.org/obo/GAZ_00030843 -->

    <owl:NamedIndividual rdf:about="http://purl.obolibrary.org/obo/GAZ_00030843">
        <obo:RO_0001025 rdf:resource="http://purl.obolibrary.org/obo/GAZ_00030835"/>
        <oboInOwl:hasOBONamespace>GAZ</oboInOwl:hasOBONamespace>
        <oboInOwl:id>GAZ:00030843</oboInOwl:id>
        <rdfs:label>Hatra District</rdfs:label>
    </owl:NamedIndividual>
    


    <!-- http://purl.obolibrary.org/obo/GAZ_00030844 -->

    <owl:NamedIndividual rdf:about="http://purl.obolibrary.org/obo/GAZ_00030844">
        <obo:RO_0001025 rdf:resource="http://purl.obolibrary.org/obo/GAZ_00030835"/>
        <oboInOwl:hasOBONamespace>GAZ</oboInOwl:hasOBONamespace>
        <oboInOwl:id>GAZ:00030844</oboInOwl:id>
        <rdfs:label>Telafar District</rdfs:label>
    </owl:NamedIndividual>
    


    <!-- http://purl.obolibrary.org/obo/GAZ_00030845 -->

    <owl:NamedIndividual rdf:about="http://purl.obolibrary.org/obo/GAZ_00030845">
        <obo:RO_0001025 rdf:resource="http://purl.obolibrary.org/obo/GAZ_00030835"/>
        <oboInOwl:hasOBONamespace>GAZ</oboInOwl:hasOBONamespace>
        <oboInOwl:id>GAZ:00030845</oboInOwl:id>
        <rdfs:label>Al-Shikhan District</rdfs:label>
    </owl:NamedIndividual>
    


    <!-- http://purl.obolibrary.org/obo/GAZ_00045681 -->

    <owl:NamedIndividual rdf:about="http://purl.obolibrary.org/obo/GAZ_00045681">
        <obo:IAO_0000115>An island that is bounded in the west by the Arvand Rud and to the east by the Bahmanshir outlet of the Karun River, 53 km from the Persian Gulf, near the Iraqi-Iran border.</obo:IAO_0000115>
        <oboInOwl:hasOBONamespace>GAZ</oboInOwl:hasOBONamespace>
        <oboInOwl:id>GAZ:00045681</oboInOwl:id>
        <rdfs:label>Abadan Island</rdfs:label>
    </owl:NamedIndividual>
    


    <!-- http://purl.obolibrary.org/obo/GAZ_00045683 -->

    <owl:NamedIndividual rdf:about="http://purl.obolibrary.org/obo/GAZ_00045683">
        <obo:RO_0001025 rdf:resource="http://purl.obolibrary.org/obo/GAZ_00250881"/>
        <obo:IAO_0000115>An island.</obo:IAO_0000115>
        <oboInOwl:hasOBONamespace>GAZ</oboInOwl:hasOBONamespace>
        <oboInOwl:id>GAZ:00045683</oboInOwl:id>
        <rdfs:label>Menak Island</rdfs:label>
    </owl:NamedIndividual>
    


    <!-- http://purl.obolibrary.org/obo/GAZ_00045685 -->

    <owl:NamedIndividual rdf:about="http://purl.obolibrary.org/obo/GAZ_00045685">
        <obo:RO_0001025 rdf:resource="http://purl.obolibrary.org/obo/GAZ_00250882"/>
        <obo:IAO_0000115>An island.</obo:IAO_0000115>
        <oboInOwl:hasOBONamespace>GAZ</oboInOwl:hasOBONamespace>
        <oboInOwl:id>GAZ:00045685</oboInOwl:id>
        <rdfs:label>Gonban Island</rdfs:label>
    </owl:NamedIndividual>
    


    <!-- http://purl.obolibrary.org/obo/GAZ_00045686 -->

    <owl:NamedIndividual rdf:about="http://purl.obolibrary.org/obo/GAZ_00045686">
        <obo:RO_0001025 rdf:resource="http://purl.obolibrary.org/obo/GAZ_00250882"/>
        <obo:IAO_0000115>An island.</obo:IAO_0000115>
        <oboInOwl:hasOBONamespace>GAZ</oboInOwl:hasOBONamespace>
        <oboInOwl:id>GAZ:00045686</oboInOwl:id>
        <rdfs:label>Narges Island</rdfs:label>
    </owl:NamedIndividual>
    


    <!-- http://purl.obolibrary.org/obo/GAZ_00045691 -->

    <owl:NamedIndividual rdf:about="http://purl.obolibrary.org/obo/GAZ_00045691">
        <obo:RO_0001025 rdf:resource="http://purl.obolibrary.org/obo/GAZ_00018525"/>
        <obo:IAO_0000115>An island.</obo:IAO_0000115>
        <oboInOwl:hasOBONamespace>GAZ</oboInOwl:hasOBONamespace>
        <oboInOwl:id>GAZ:00045691</oboInOwl:id>
        <rdfs:label>Greater Tunb</rdfs:label>
    </owl:NamedIndividual>
    


    <!-- http://purl.obolibrary.org/obo/GAZ_00045692 -->

    <owl:NamedIndividual rdf:about="http://purl.obolibrary.org/obo/GAZ_00045692">
        <obo:RO_0001025 rdf:resource="http://purl.obolibrary.org/obo/GAZ_00018525"/>
        <obo:IAO_0000115>An island.</obo:IAO_0000115>
        <oboInOwl:hasOBONamespace>GAZ</oboInOwl:hasOBONamespace>
        <oboInOwl:id>GAZ:00045692</oboInOwl:id>
        <rdfs:label>Lesser Tunb</rdfs:label>
    </owl:NamedIndividual>
    


    <!-- http://purl.obolibrary.org/obo/GAZ_00047079 -->

    <owl:NamedIndividual rdf:about="http://purl.obolibrary.org/obo/GAZ_00047079">
        <obo:RO_0001025 rdf:resource="http://purl.obolibrary.org/obo/GAZ_00005295"/>
        <obo:IAO_0000115>An offshore Island in the Persian Gulf.</obo:IAO_0000115>
        <oboInOwl:hasOBONamespace>GAZ</oboInOwl:hasOBONamespace>
        <oboInOwl:id>GAZ:00047079</oboInOwl:id>
        <rdfs:label>Das</rdfs:label>
    </owl:NamedIndividual>
    


    <!-- http://purl.obolibrary.org/obo/GAZ_00047080 -->

    <owl:NamedIndividual rdf:about="http://purl.obolibrary.org/obo/GAZ_00047080">
        <obo:RO_0001025 rdf:resource="http://purl.obolibrary.org/obo/GAZ_00005295"/>
        <obo:IAO_0000115>An island off the coast of Abu Dhabi, United Arab Emirates.</obo:IAO_0000115>
        <oboInOwl:hasOBONamespace>GAZ</oboInOwl:hasOBONamespace>
        <oboInOwl:id>GAZ:00047080</oboInOwl:id>
        <rdfs:label>Dalma Island</rdfs:label>
    </owl:NamedIndividual>
    


    <!-- http://purl.obolibrary.org/obo/GAZ_00047081 -->

    <owl:NamedIndividual rdf:about="http://purl.obolibrary.org/obo/GAZ_00047081">
        <obo:RO_0001025 rdf:resource="http://purl.obolibrary.org/obo/GAZ_00005295"/>
        <obo:IAO_0000115>An island.</obo:IAO_0000115>
        <oboInOwl:hasOBONamespace>GAZ</oboInOwl:hasOBONamespace>
        <oboInOwl:id>GAZ:00047081</oboInOwl:id>
        <rdfs:label>Arzanah Island</rdfs:label>
    </owl:NamedIndividual>
    


    <!-- http://purl.obolibrary.org/obo/GAZ_00048421 -->

    <owl:NamedIndividual rdf:about="http://purl.obolibrary.org/obo/GAZ_00048421">
        <obo:RO_0001025 rdf:resource="http://purl.obolibrary.org/obo/GAZ_00006936"/>
        <oboInOwl:hasOBONamespace>GAZ</oboInOwl:hasOBONamespace>
        <oboInOwl:id>GAZ:00048421</oboInOwl:id>
        <rdfs:label>Al Hidd Island</rdfs:label>
    </owl:NamedIndividual>
    


    <!-- http://purl.obolibrary.org/obo/GAZ_00049020 -->

    <owl:NamedIndividual rdf:about="http://purl.obolibrary.org/obo/GAZ_00049020">
        <obo:RO_0001025 rdf:resource="http://purl.obolibrary.org/obo/GAZ_00005295"/>
        <obo:IAO_0000115>The largest of about 200 islands along the coast of the United Arab Emirates. It is situated in the emirate of Abu Dhabi.</obo:IAO_0000115>
        <oboInOwl:hasOBONamespace>GAZ</oboInOwl:hasOBONamespace>
        <oboInOwl:id>GAZ:00049020</oboInOwl:id>
        <rdfs:label>Abu al Abyad</rdfs:label>
    </owl:NamedIndividual>
    


    <!-- http://purl.obolibrary.org/obo/GAZ_00052482 -->

    <owl:NamedIndividual rdf:about="http://purl.obolibrary.org/obo/GAZ_00052482">
        <obo:RO_0001025 rdf:resource="http://purl.obolibrary.org/obo/GAZ_00030494"/>
    </owl:NamedIndividual>
    


    <!-- http://purl.obolibrary.org/obo/GAZ_00052483 -->

    <owl:NamedIndividual rdf:about="http://purl.obolibrary.org/obo/GAZ_00052483">
        <obo:RO_0001025 rdf:resource="http://purl.obolibrary.org/obo/GAZ_00030465"/>
    </owl:NamedIndividual>
    


    <!-- http://purl.obolibrary.org/obo/GAZ_00052484 -->

    <owl:NamedIndividual rdf:about="http://purl.obolibrary.org/obo/GAZ_00052484">
        <obo:RO_0001025 rdf:resource="http://purl.obolibrary.org/obo/GAZ_00030447"/>
    </owl:NamedIndividual>
    


    <!-- http://purl.obolibrary.org/obo/GAZ_00052485 -->

    <owl:NamedIndividual rdf:about="http://purl.obolibrary.org/obo/GAZ_00052485">
        <obo:RO_0001025 rdf:resource="http://purl.obolibrary.org/obo/GAZ_00030835"/>
        <obo:IAO_0000115>Mountains N of the alluvial plains, between the Tigris and the Euphrates rivers, is the arid Al-Jazirah plateau. Its most prominent hill range is the Sinjar Mountains, whose highest peak reaches an elevation of 1,356 m. The main watercourse is the Wadi Al-Tharthar, which runs southward for 210 km from the Sinjar Mountains to the Tharthar.</obo:IAO_0000115>
        <oboInOwl:hasOBONamespace>GAZ</oboInOwl:hasOBONamespace>
        <oboInOwl:id>GAZ:00052485</oboInOwl:id>
        <rdfs:label>Jabal Sinjar</rdfs:label>
    </owl:NamedIndividual>
    


    <!-- http://purl.obolibrary.org/obo/GAZ_00052486 -->

    <owl:NamedIndividual rdf:about="http://purl.obolibrary.org/obo/GAZ_00052486">
        <obo:RO_0001025 rdf:resource="http://purl.obolibrary.org/obo/GAZ_00030822"/>
    </owl:NamedIndividual>
    


    <!-- http://purl.obolibrary.org/obo/GAZ_00052487 -->

    <owl:NamedIndividual rdf:about="http://purl.obolibrary.org/obo/GAZ_00052487">
        <obo:RO_0001025 rdf:resource="http://purl.obolibrary.org/obo/GAZ_00030818"/>
    </owl:NamedIndividual>
    


    <!-- http://purl.obolibrary.org/obo/GAZ_00052488 -->

    <owl:NamedIndividual rdf:about="http://purl.obolibrary.org/obo/GAZ_00052488">
        <obo:RO_0001025 rdf:resource="http://purl.obolibrary.org/obo/GAZ_00030465"/>
    </owl:NamedIndividual>
    


    <!-- http://purl.obolibrary.org/obo/GAZ_00053728 -->

    <owl:NamedIndividual rdf:about="http://purl.obolibrary.org/obo/GAZ_00053728">
        <obo:RO_0001025 rdf:resource="http://purl.obolibrary.org/obo/GAZ_00005295"/>
        <obo:IAO_0000115>An island in the Persian Gulf.</obo:IAO_0000115>
        <oboInOwl:hasOBONamespace>GAZ</oboInOwl:hasOBONamespace>
        <oboInOwl:id>GAZ:00053728</oboInOwl:id>
        <rdfs:label>Shidvar Island</rdfs:label>
    </owl:NamedIndividual>
    


    <!-- http://purl.obolibrary.org/obo/GAZ_00053729 -->

    <owl:NamedIndividual rdf:about="http://purl.obolibrary.org/obo/GAZ_00053729">
        <obo:RO_0001025 rdf:resource="http://purl.obolibrary.org/obo/GAZ_00045681"/>
    </owl:NamedIndividual>
    


    <!-- http://purl.obolibrary.org/obo/GAZ_00057473 -->

    <owl:NamedIndividual rdf:about="http://purl.obolibrary.org/obo/GAZ_00057473">
        <obo:RO_0001025 rdf:resource="http://purl.obolibrary.org/obo/GAZ_02000626"/>
        <obo:IAO_0000115>A man-made saline lake WSW of Bagdad. Lake Milh is a depression into which excess water from the Euphrates River is diverted by a controlled escape channel or canal. The lake is rather shallow and water levels change with the seasons. Constructed 1970s.</obo:IAO_0000115>
        <oboInOwl:hasOBONamespace>GAZ</oboInOwl:hasOBONamespace>
        <oboInOwl:id>GAZ:00057473</oboInOwl:id>
        <rdfs:label>Lake Milh</rdfs:label>
    </owl:NamedIndividual>
    


    <!-- http://purl.obolibrary.org/obo/GAZ_00057474 -->

    <owl:NamedIndividual rdf:about="http://purl.obolibrary.org/obo/GAZ_00057474">
        <obo:RO_0001025 rdf:resource="http://purl.obolibrary.org/obo/GAZ_02000627"/>
        <obo:IAO_0000115>A shallow natural lake in al-Anbar, Iraq, west of Baghdad. It has a surface area 140 km2. Traditionally the lake has been used to hold flood water from the River Euphrates, and in 1956 a barrage was constructed at Ramadi for this purpose.</obo:IAO_0000115>
        <oboInOwl:hasOBONamespace>GAZ</oboInOwl:hasOBONamespace>
        <oboInOwl:id>GAZ:00057474</oboInOwl:id>
        <rdfs:label>Lake Habbaniyah</rdfs:label>
    </owl:NamedIndividual>
    


    <!-- http://purl.obolibrary.org/obo/GAZ_00057475 -->

    <owl:NamedIndividual rdf:about="http://purl.obolibrary.org/obo/GAZ_00057475">
        <obo:RO_0001025 rdf:resource="http://purl.obolibrary.org/obo/GAZ_02000616"/>
        <obo:IAO_0000115>A brackish (formerly saline) lake situated 120 km north of Baghdad between the Tigris and the Euphrates rivers.</obo:IAO_0000115>
        <oboInOwl:hasOBONamespace>GAZ</oboInOwl:hasOBONamespace>
        <oboInOwl:id>GAZ:00057475</oboInOwl:id>
        <rdfs:label>Lake Tharthar</rdfs:label>
    </owl:NamedIndividual>
    


    <!-- http://purl.obolibrary.org/obo/GAZ_00057476 -->

    <owl:NamedIndividual rdf:about="http://purl.obolibrary.org/obo/GAZ_00057476">
        <obo:RO_0001025 rdf:resource="http://purl.obolibrary.org/obo/GAZ_00004483"/>
        <obo:IAO_0000115>An autonomous, federally recognized political, ethnic and economic region of Iraqn. It borders Iranian Kurdistan to the east, Turkish Kurdistan to the north, Syrian Kurdistan to the west and Iraqi Kurdistan to the south. Its capital is the city of Arbil.</obo:IAO_0000115>
        <oboInOwl:hasOBONamespace>GAZ</oboInOwl:hasOBONamespace>
        <oboInOwl:id>GAZ:00057476</oboInOwl:id>
        <rdfs:label>Kurdistan Region</rdfs:label>
    </owl:NamedIndividual>
    


    <!-- http://purl.obolibrary.org/obo/GAZ_00057477 -->

    <owl:NamedIndividual rdf:about="http://purl.obolibrary.org/obo/GAZ_00057477">
        <obo:RO_0001025 rdf:resource="http://purl.obolibrary.org/obo/GAZ_02000620"/>
        <obo:IAO_0000115>A mountain range in Iraq that extend from Diyala province, 60 km east of Baghdad, and borders on Iran and extend to oil rich city of Kirkuk, 260 km north of Baghdad.</obo:IAO_0000115>
        <oboInOwl:hasOBONamespace>GAZ</oboInOwl:hasOBONamespace>
        <oboInOwl:id>GAZ:00057477</oboInOwl:id>
        <rdfs:label>Hamrin Range</rdfs:label>
    </owl:NamedIndividual>
    


    <!-- http://purl.obolibrary.org/obo/GAZ_00058254 -->

    <owl:NamedIndividual rdf:about="http://purl.obolibrary.org/obo/GAZ_00058254">
        <obo:RO_0001025 rdf:resource="http://purl.obolibrary.org/obo/GAZ_00057476"/>
        <obo:IAO_0000115>A lake in Kurdistan Region which lies in northeastern Iraq. The lake is close to the city of Rania.</obo:IAO_0000115>
        <oboInOwl:hasOBONamespace>GAZ</oboInOwl:hasOBONamespace>
        <oboInOwl:id>GAZ:00058254</oboInOwl:id>
        <rdfs:label>Lake Dukan</rdfs:label>
    </owl:NamedIndividual>
    


    <!-- http://purl.obolibrary.org/obo/GAZ_00058255 -->

    <owl:NamedIndividual rdf:about="http://purl.obolibrary.org/obo/GAZ_00058255">
        <obo:RO_0001025 rdf:resource="http://purl.obolibrary.org/obo/GAZ_00193962"/>
        <obo:IAO_0000115>A saline lake in southeastern part of Iraq.</obo:IAO_0000115>
        <oboInOwl:hasOBONamespace>GAZ</oboInOwl:hasOBONamespace>
        <oboInOwl:id>GAZ:00058255</oboInOwl:id>
        <rdfs:label>Lake Hammar</rdfs:label>
    </owl:NamedIndividual>
    


    <!-- http://purl.obolibrary.org/obo/GAZ_00058256 -->

    <owl:NamedIndividual rdf:about="http://purl.obolibrary.org/obo/GAZ_00058256">
        <obo:RO_0001025 rdf:resource="http://purl.obolibrary.org/obo/GAZ_00193963"/>
        <obo:IAO_0000115>A freshwater lake in the Al Amarah marshes of southern Iraq. The 3.4 km wide lake is approximately 17 km north of the Tigris-Euphrates confluence. Because of it&apos;s shape and location, it is believed to be a Holocene bolide impact crater.</obo:IAO_0000115>
        <oboInOwl:hasOBONamespace>GAZ</oboInOwl:hasOBONamespace>
        <oboInOwl:id>GAZ:00058256</oboInOwl:id>
        <rdfs:label>Umm al Binni Lake</rdfs:label>
    </owl:NamedIndividual>
    


    <!-- http://purl.obolibrary.org/obo/GAZ_00062456 -->

    <owl:NamedIndividual rdf:about="http://purl.obolibrary.org/obo/GAZ_00062456">
        <obo:IAO_0000115>A water storage reservoir. A large lake in Syria on the Euphrates River; a body of water about 80 km long and averaging eight km in width created by the Tabaqah Dam.</obo:IAO_0000115>
        <oboInOwl:hasOBONamespace>GAZ</oboInOwl:hasOBONamespace>
        <oboInOwl:id>GAZ:00062456</oboInOwl:id>
        <rdfs:label>Buhayrat al Asad</rdfs:label>
    </owl:NamedIndividual>
    


    <!-- http://purl.obolibrary.org/obo/GAZ_00078574 -->

    <owl:NamedIndividual rdf:about="http://purl.obolibrary.org/obo/GAZ_00078574">
        <obo:RO_0001025 rdf:resource="http://purl.obolibrary.org/obo/GAZ_00005295"/>
        <obo:IAO_0000115>A natural island 600 m off the coast of Abu Dhabi island.</obo:IAO_0000115>
        <oboInOwl:hasOBONamespace>GAZ</oboInOwl:hasOBONamespace>
        <oboInOwl:id>GAZ:00078574</oboInOwl:id>
        <rdfs:label>Al Reem Island</rdfs:label>
    </owl:NamedIndividual>
    


    <!-- http://purl.obolibrary.org/obo/GAZ_00078575 -->

    <owl:NamedIndividual rdf:about="http://purl.obolibrary.org/obo/GAZ_00078575">
        <obo:RO_0001025 rdf:resource="http://purl.obolibrary.org/obo/GAZ_00005295"/>
        <obo:IAO_0000115>A large, low lying island 500 m off the coast of Abu Dhabi island.</obo:IAO_0000115>
        <oboInOwl:hasOBONamespace>GAZ</oboInOwl:hasOBONamespace>
        <oboInOwl:id>GAZ:00078575</oboInOwl:id>
        <rdfs:label>Saadiyat Island</rdfs:label>
    </owl:NamedIndividual>
    


    <!-- http://purl.obolibrary.org/obo/GAZ_00078576 -->

    <owl:NamedIndividual rdf:about="http://purl.obolibrary.org/obo/GAZ_00078576">
        <obo:RO_0001025 rdf:resource="http://purl.obolibrary.org/obo/GAZ_00005295"/>
        <oboInOwl:hasOBONamespace>GAZ</oboInOwl:hasOBONamespace>
        <oboInOwl:id>GAZ:00078576</oboInOwl:id>
        <rdfs:label>Abu Dhabi Island</rdfs:label>
    </owl:NamedIndividual>
    


    <!-- http://purl.obolibrary.org/obo/GAZ_00078583 -->

    <owl:NamedIndividual rdf:about="http://purl.obolibrary.org/obo/GAZ_00078583">
        <obo:RO_0001025 rdf:resource="http://purl.obolibrary.org/obo/GAZ_00005295"/>
        <obo:IAO_0000115>A mangrove island S of Kalba.</obo:IAO_0000115>
        <oboInOwl:hasOBONamespace>GAZ</oboInOwl:hasOBONamespace>
        <oboInOwl:id>GAZ:00078583</oboInOwl:id>
        <rdfs:label>Khor Kalba</rdfs:label>
    </owl:NamedIndividual>
    


    <!-- http://purl.obolibrary.org/obo/GAZ_00078658 -->

    <owl:NamedIndividual rdf:about="http://purl.obolibrary.org/obo/GAZ_00078658">
        <rdf:type rdf:resource="http://purl.obolibrary.org/obo/ENVO_00000856"/>
        <obo:RO_0001025 rdf:resource="http://purl.obolibrary.org/obo/GAZ_02000358"/>
        <obo:RO_0001025 rdf:resource="http://purl.obolibrary.org/obo/GAZ_02000360"/>
        <obo:IAO_0000115>A municipality in the Northern and Southern Governorates.</obo:IAO_0000115>
        <oboInOwl:hasOBONamespace>GAZ</oboInOwl:hasOBONamespace>
        <oboInOwl:id>GAZ:00078658</oboInOwl:id>
        <rdfs:label>Municipality of Al Mintaqah al Gharbiyah</rdfs:label>
    </owl:NamedIndividual>
    


    <!-- http://purl.obolibrary.org/obo/GAZ_00078659 -->

    <owl:NamedIndividual rdf:about="http://purl.obolibrary.org/obo/GAZ_00078659">
        <rdf:type rdf:resource="http://purl.obolibrary.org/obo/ENVO_00000856"/>
        <obo:RO_0001025 rdf:resource="http://purl.obolibrary.org/obo/GAZ_02000358"/>
        <obo:RO_0001025 rdf:resource="http://purl.obolibrary.org/obo/GAZ_02000361"/>
        <obo:IAO_0000115>A municipality in the Central and Southern Governorates.</obo:IAO_0000115>
        <oboInOwl:hasOBONamespace>GAZ</oboInOwl:hasOBONamespace>
        <oboInOwl:id>GAZ:00078659</oboInOwl:id>
        <rdfs:label>Municipality of Ar Rifa&apos; wa al Mintaqah al Janubiyah</rdfs:label>
    </owl:NamedIndividual>
    


    <!-- http://purl.obolibrary.org/obo/GAZ_00078660 -->

    <owl:NamedIndividual rdf:about="http://purl.obolibrary.org/obo/GAZ_00078660">
        <obo:RO_0001025 rdf:resource="http://purl.obolibrary.org/obo/GAZ_02000358"/>
        <oboInOwl:hasOBONamespace>GAZ</oboInOwl:hasOBONamespace>
        <oboInOwl:id>GAZ:00078660</oboInOwl:id>
        <rdfs:label>Municipality of Juzur Hawar</rdfs:label>
    </owl:NamedIndividual>
    


    <!-- http://purl.obolibrary.org/obo/GAZ_00078661 -->

    <owl:NamedIndividual rdf:about="http://purl.obolibrary.org/obo/GAZ_00078661">
        <obo:RO_0001025 rdf:resource="http://purl.obolibrary.org/obo/GAZ_00005295"/>
        <obo:RO_0001025 rdf:resource="http://purl.obolibrary.org/obo/GAZ_00006936"/>
        <obo:RO_0001025 rdf:resource="http://purl.obolibrary.org/obo/GAZ_00078660"/>
        <obo:IAO_0000115>A group of islands situated off the west coast of Qatar in the Gulf of Bahrain of the Persian Gulf. Despite their proximity to Qatar (Suwad al Janubiyah is only 1.4 km from the Qatari mainland at the peninsula of Ras Abruq, while Rubud Al Gharbiyah, the island closest to the main island of Bahrain, lies at a distance of 19.7 km to it), the islands belong to Bahrain. A Ramsar Site.</obo:IAO_0000115>
        <oboInOwl:hasOBONamespace>GAZ</oboInOwl:hasOBONamespace>
        <oboInOwl:id>GAZ:00078661</oboInOwl:id>
        <rdfs:label>Hawar Islands</rdfs:label>
    </owl:NamedIndividual>
    


    <!-- http://purl.obolibrary.org/obo/GAZ_00078662 -->

    <owl:NamedIndividual rdf:about="http://purl.obolibrary.org/obo/GAZ_00078662">
        <obo:RO_0001025 rdf:resource="http://purl.obolibrary.org/obo/GAZ_00078661"/>
        <obo:IAO_0000115>An island in the Hawar Islands.</obo:IAO_0000115>
        <oboInOwl:hasOBONamespace>GAZ</oboInOwl:hasOBONamespace>
        <oboInOwl:id>GAZ:00078662</oboInOwl:id>
        <rdfs:label>Rubud Al Gharbiyah</rdfs:label>
    </owl:NamedIndividual>
    


    <!-- http://purl.obolibrary.org/obo/GAZ_00078663 -->

    <owl:NamedIndividual rdf:about="http://purl.obolibrary.org/obo/GAZ_00078663">
        <obo:RO_0001025 rdf:resource="http://purl.obolibrary.org/obo/GAZ_00078661"/>
        <obo:IAO_0000115>An island in the Hawar Islands.</obo:IAO_0000115>
        <oboInOwl:hasOBONamespace>GAZ</oboInOwl:hasOBONamespace>
        <oboInOwl:id>GAZ:00078663</oboInOwl:id>
        <rdfs:label>Rubud Al Sharqiyah</rdfs:label>
    </owl:NamedIndividual>
    


    <!-- http://purl.obolibrary.org/obo/GAZ_00078664 -->

    <owl:NamedIndividual rdf:about="http://purl.obolibrary.org/obo/GAZ_00078664">
        <obo:RO_0001025 rdf:resource="http://purl.obolibrary.org/obo/GAZ_00078661"/>
        <obo:IAO_0000115>An island in the Hawar Islands.</obo:IAO_0000115>
        <oboInOwl:hasOBONamespace>GAZ</oboInOwl:hasOBONamespace>
        <oboInOwl:id>GAZ:00078664</oboInOwl:id>
        <rdfs:label>Umm Jinni</rdfs:label>
    </owl:NamedIndividual>
    


    <!-- http://purl.obolibrary.org/obo/GAZ_00078665 -->

    <owl:NamedIndividual rdf:about="http://purl.obolibrary.org/obo/GAZ_00078665">
        <obo:RO_0001025 rdf:resource="http://purl.obolibrary.org/obo/GAZ_00078661"/>
        <obo:IAO_0000115>A group of islands in the Hawar Islands.</obo:IAO_0000115>
        <oboInOwl:hasOBONamespace>GAZ</oboInOwl:hasOBONamespace>
        <oboInOwl:id>GAZ:00078665</oboInOwl:id>
        <rdfs:label>Al Hajiyat</rdfs:label>
    </owl:NamedIndividual>
    


    <!-- http://purl.obolibrary.org/obo/GAZ_00078666 -->

    <owl:NamedIndividual rdf:about="http://purl.obolibrary.org/obo/GAZ_00078666">
        <obo:RO_0001025 rdf:resource="http://purl.obolibrary.org/obo/GAZ_00078661"/>
        <obo:IAO_0000115>An island in the Hawar Islands.</obo:IAO_0000115>
        <oboInOwl:hasOBONamespace>GAZ</oboInOwl:hasOBONamespace>
        <oboInOwl:id>GAZ:00078666</oboInOwl:id>
        <rdfs:label>Ajirah</rdfs:label>
    </owl:NamedIndividual>
    


    <!-- http://purl.obolibrary.org/obo/GAZ_00078667 -->

    <owl:NamedIndividual rdf:about="http://purl.obolibrary.org/obo/GAZ_00078667">
        <obo:RO_0001025 rdf:resource="http://purl.obolibrary.org/obo/GAZ_00078661"/>
        <obo:IAO_0000115>An island in the Hawar Islands.</obo:IAO_0000115>
        <oboInOwl:hasOBONamespace>GAZ</oboInOwl:hasOBONamespace>
        <oboInOwl:id>GAZ:00078667</oboInOwl:id>
        <rdfs:label>Suwad al Janubiyah</rdfs:label>
    </owl:NamedIndividual>
    


    <!-- http://purl.obolibrary.org/obo/GAZ_00078668 -->

    <owl:NamedIndividual rdf:about="http://purl.obolibrary.org/obo/GAZ_00078668">
        <obo:RO_0001025 rdf:resource="http://purl.obolibrary.org/obo/GAZ_00078661"/>
        <obo:IAO_0000115>An island in the Hawar Islands.</obo:IAO_0000115>
        <oboInOwl:hasOBONamespace>GAZ</oboInOwl:hasOBONamespace>
        <oboInOwl:id>GAZ:00078668</oboInOwl:id>
        <rdfs:label>Umm Kharurah</rdfs:label>
    </owl:NamedIndividual>
    


    <!-- http://purl.obolibrary.org/obo/GAZ_00078669 -->

    <owl:NamedIndividual rdf:about="http://purl.obolibrary.org/obo/GAZ_00078669">
        <obo:RO_0001025 rdf:resource="http://purl.obolibrary.org/obo/GAZ_00078661"/>
        <obo:IAO_0000115>Isolated sea stacks with shingle beaches with surrounding shallow lagoon in the Hawar Islands.</obo:IAO_0000115>
        <oboInOwl:hasOBONamespace>GAZ</oboInOwl:hasOBONamespace>
        <oboInOwl:id>GAZ:00078669</oboInOwl:id>
        <rdfs:label>al Wukur</rdfs:label>
    </owl:NamedIndividual>
    


    <!-- http://purl.obolibrary.org/obo/GAZ_00078670 -->

    <owl:NamedIndividual rdf:about="http://purl.obolibrary.org/obo/GAZ_00078670">
        <obo:RO_0001025 rdf:resource="http://purl.obolibrary.org/obo/GAZ_00078661"/>
        <obo:IAO_0000115>A group of islands in the Hawar Islands.</obo:IAO_0000115>
        <oboInOwl:hasOBONamespace>GAZ</oboInOwl:hasOBONamespace>
        <oboInOwl:id>GAZ:00078670</oboInOwl:id>
        <rdfs:label>Bu Tammur</rdfs:label>
    </owl:NamedIndividual>
    


    <!-- http://purl.obolibrary.org/obo/GAZ_00078671 -->

    <owl:NamedIndividual rdf:about="http://purl.obolibrary.org/obo/GAZ_00078671">
        <obo:RO_0001025 rdf:resource="http://purl.obolibrary.org/obo/GAZ_00078661"/>
        <obo:IAO_0000115>An island in the Hawar Islands.</obo:IAO_0000115>
        <oboInOwl:hasOBONamespace>GAZ</oboInOwl:hasOBONamespace>
        <oboInOwl:id>GAZ:00078671</oboInOwl:id>
        <rdfs:label>Muhazwarah</rdfs:label>
    </owl:NamedIndividual>
    


    <!-- http://purl.obolibrary.org/obo/GAZ_00078672 -->

    <owl:NamedIndividual rdf:about="http://purl.obolibrary.org/obo/GAZ_00078672">
        <obo:RO_0001025 rdf:resource="http://purl.obolibrary.org/obo/GAZ_00078661"/>
        <obo:IAO_0000115>An island in the Hawar Islands.</obo:IAO_0000115>
        <oboInOwl:hasOBONamespace>GAZ</oboInOwl:hasOBONamespace>
        <oboInOwl:id>GAZ:00078672</oboInOwl:id>
        <rdfs:label>Suwad ash Shamaliyah</rdfs:label>
    </owl:NamedIndividual>
    


    <!-- http://purl.obolibrary.org/obo/GAZ_00078673 -->

    <owl:NamedIndividual rdf:about="http://purl.obolibrary.org/obo/GAZ_00078673">
        <obo:RO_0001025 rdf:resource="http://purl.obolibrary.org/obo/GAZ_00078661"/>
        <obo:IAO_0000115>A group of islands in the Hawar Islands.</obo:IAO_0000115>
        <oboInOwl:hasOBONamespace>GAZ</oboInOwl:hasOBONamespace>
        <oboInOwl:id>GAZ:00078673</oboInOwl:id>
        <rdfs:label>Bu Sadad</rdfs:label>
    </owl:NamedIndividual>
    


    <!-- http://purl.obolibrary.org/obo/GAZ_00078674 -->

    <owl:NamedIndividual rdf:about="http://purl.obolibrary.org/obo/GAZ_00078674">
        <obo:RO_0001025 rdf:resource="http://purl.obolibrary.org/obo/GAZ_00078661"/>
        <obo:IAO_0000115>An island in the Hawar Islands.</obo:IAO_0000115>
        <oboInOwl:hasOBONamespace>GAZ</oboInOwl:hasOBONamespace>
        <oboInOwl:id>GAZ:00078674</oboInOwl:id>
        <rdfs:label>Jazirat Jinan</rdfs:label>
    </owl:NamedIndividual>
    


    <!-- http://purl.obolibrary.org/obo/GAZ_00078675 -->

    <owl:NamedIndividual rdf:about="http://purl.obolibrary.org/obo/GAZ_00078675">
        <rdf:type rdf:resource="http://purl.obolibrary.org/obo/ENVO_00000856"/>
        <obo:RO_0001025 rdf:resource="http://purl.obolibrary.org/obo/GAZ_02000360"/>
        <obo:RO_0001025 rdf:resource="http://purl.obolibrary.org/obo/GAZ_02000361"/>
        <obo:IAO_0000115>A municipality of Bahrain in the northern part of the country. Its territory is now in the Central and Northern Governorates.</obo:IAO_0000115>
        <oboInOwl:hasOBONamespace>GAZ</oboInOwl:hasOBONamespace>
        <oboInOwl:id>GAZ:00078675</oboInOwl:id>
        <rdfs:label>Municipality of Al Mintaqah al Wusta</rdfs:label>
    </owl:NamedIndividual>
    


    <!-- http://purl.obolibrary.org/obo/GAZ_00078676 -->

    <owl:NamedIndividual rdf:about="http://purl.obolibrary.org/obo/GAZ_00078676">
        <rdf:type rdf:resource="http://purl.obolibrary.org/obo/ENVO_00000856"/>
        <obo:RO_0001025 rdf:resource="http://purl.obolibrary.org/obo/GAZ_02000360"/>
        <obo:RO_0001025 rdf:resource="http://purl.obolibrary.org/obo/GAZ_02000362"/>
        <obo:IAO_0000115>A municipality in northern Bahrain. It was split off of the municipality of Ar Rifa&apos; wa al Mintaqah al Janubiyah in 1991.</obo:IAO_0000115>
        <oboInOwl:hasOBONamespace>GAZ</oboInOwl:hasOBONamespace>
        <oboInOwl:id>GAZ:00078676</oboInOwl:id>
        <rdfs:label>Municipality of Madinat Hamad</rdfs:label>
    </owl:NamedIndividual>
    


    <!-- http://purl.obolibrary.org/obo/GAZ_00078677 -->

    <owl:NamedIndividual rdf:about="http://purl.obolibrary.org/obo/GAZ_00078677">
        <rdf:type rdf:resource="http://purl.obolibrary.org/obo/ENVO_00000856"/>
        <obo:RO_0001025 rdf:resource="http://purl.obolibrary.org/obo/GAZ_02000360"/>
        <obo:RO_0001025 rdf:resource="http://purl.obolibrary.org/obo/GAZ_02000362"/>
        <obo:IAO_0000115>A municipality in northern Bahrain. Now in the Capital and Northern Governorate.</obo:IAO_0000115>
        <oboInOwl:hasOBONamespace>GAZ</oboInOwl:hasOBONamespace>
        <oboInOwl:id>GAZ:00078677</oboInOwl:id>
        <rdfs:label>Municipality of Jidd Haffs</rdfs:label>
    </owl:NamedIndividual>
    


    <!-- http://purl.obolibrary.org/obo/GAZ_00078678 -->

    <owl:NamedIndividual rdf:about="http://purl.obolibrary.org/obo/GAZ_00078678">
        <rdf:type rdf:resource="http://purl.obolibrary.org/obo/ENVO_00000856"/>
        <obo:RO_0001025 rdf:resource="http://purl.obolibrary.org/obo/GAZ_02000360"/>
        <obo:IAO_0000115>A municipality of Bahrain in the northern part of the country. Its territory is now in the Northern Governorate.</obo:IAO_0000115>
        <oboInOwl:hasOBONamespace>GAZ</oboInOwl:hasOBONamespace>
        <oboInOwl:id>GAZ:00078678</oboInOwl:id>
        <rdfs:label>Municipality of Al Mintaqah al Shamaliyah</rdfs:label>
    </owl:NamedIndividual>
    


    <!-- http://purl.obolibrary.org/obo/GAZ_00078679 -->

    <owl:NamedIndividual rdf:about="http://purl.obolibrary.org/obo/GAZ_00078679">
        <obo:RO_0001025 rdf:resource="http://purl.obolibrary.org/obo/GAZ_00078676"/>
        <obo:IAO_0000115>The capital city of Bahrain.</obo:IAO_0000115>
        <oboInOwl:hasOBONamespace>GAZ</oboInOwl:hasOBONamespace>
        <oboInOwl:id>GAZ:00078679</oboInOwl:id>
        <rdfs:label>Manama</rdfs:label>
    </owl:NamedIndividual>
    


    <!-- http://purl.obolibrary.org/obo/GAZ_00078680 -->

    <owl:NamedIndividual rdf:about="http://purl.obolibrary.org/obo/GAZ_00078680">
        <rdf:type rdf:resource="http://purl.obolibrary.org/obo/ENVO_00000856"/>
        <obo:RO_0001025 rdf:resource="http://purl.obolibrary.org/obo/GAZ_02000359"/>
        <obo:IAO_0000115>A municipality in the Al Muharraq Governorate.</obo:IAO_0000115>
        <oboInOwl:hasOBONamespace>GAZ</oboInOwl:hasOBONamespace>
        <oboInOwl:id>GAZ:00078680</oboInOwl:id>
        <rdfs:label>Municipality of Al Muharraq</rdfs:label>
    </owl:NamedIndividual>
    


    <!-- http://purl.obolibrary.org/obo/GAZ_00078681 -->

    <owl:NamedIndividual rdf:about="http://purl.obolibrary.org/obo/GAZ_00078681">
        <rdf:type rdf:resource="http://purl.obolibrary.org/obo/ENVO_00000856"/>
        <obo:RO_0001025 rdf:resource="http://purl.obolibrary.org/obo/GAZ_02000359"/>
        <obo:IAO_0000115>A small municipality of Bahrain in the northeastern part of the country. Its territory is now in the Muharraq Governorate.</obo:IAO_0000115>
        <oboInOwl:hasOBONamespace>GAZ</oboInOwl:hasOBONamespace>
        <oboInOwl:id>GAZ:00078681</oboInOwl:id>
        <rdfs:label>Municipality of Al Hadd</rdfs:label>
    </owl:NamedIndividual>
    


    <!-- http://purl.obolibrary.org/obo/GAZ_00078682 -->

    <owl:NamedIndividual rdf:about="http://purl.obolibrary.org/obo/GAZ_00078682">
        <obo:RO_0001025 rdf:resource="http://purl.obolibrary.org/obo/GAZ_00078680"/>
        <obo:IAO_0000115>A man-made island near Al Muharraq.</obo:IAO_0000115>
        <oboInOwl:hasOBONamespace>GAZ</oboInOwl:hasOBONamespace>
        <oboInOwl:id>GAZ:00078682</oboInOwl:id>
        <rdfs:label>AMWAJ Island</rdfs:label>
    </owl:NamedIndividual>
    


    <!-- http://purl.obolibrary.org/obo/GAZ_00078683 -->

    <owl:NamedIndividual rdf:about="http://purl.obolibrary.org/obo/GAZ_00078683">
        <rdf:type rdf:resource="http://purl.obolibrary.org/obo/ENVO_00000856"/>
        <obo:RO_0001025 rdf:resource="http://purl.obolibrary.org/obo/GAZ_00006940"/>
        <obo:RO_0001025 rdf:resource="http://purl.obolibrary.org/obo/GAZ_02000361"/>
        <obo:IAO_0000115>A municipality in northeastern Bahrain. The region of Sitrah consists of the island of Sitrah and three villages close to it on the main island of Bahrain.</obo:IAO_0000115>
        <oboInOwl:hasOBONamespace>GAZ</oboInOwl:hasOBONamespace>
        <oboInOwl:id>GAZ:00078683</oboInOwl:id>
        <rdfs:label>Municipality of Sitrah</rdfs:label>
    </owl:NamedIndividual>
    


    <!-- http://purl.obolibrary.org/obo/GAZ_00078684 -->

    <owl:NamedIndividual rdf:about="http://purl.obolibrary.org/obo/GAZ_00078684">
        <rdf:type rdf:resource="http://purl.obolibrary.org/obo/ENVO_00000856"/>
        <obo:RO_0001025 rdf:resource="http://purl.obolibrary.org/obo/GAZ_02000361"/>
        <obo:IAO_0000115>A municipality located in the middle of Bahrain island, south of Isa town and north of Riffa.</obo:IAO_0000115>
        <oboInOwl:hasOBONamespace>GAZ</oboInOwl:hasOBONamespace>
        <oboInOwl:id>GAZ:00078684</oboInOwl:id>
        <rdfs:label>Municipality of A&apos;ali</rdfs:label>
    </owl:NamedIndividual>
    


    <!-- http://purl.obolibrary.org/obo/GAZ_00078685 -->

    <owl:NamedIndividual rdf:about="http://purl.obolibrary.org/obo/GAZ_00078685">
        <rdf:type rdf:resource="http://purl.obolibrary.org/obo/ENVO_00000856"/>
        <obo:RO_0001025 rdf:resource="http://purl.obolibrary.org/obo/GAZ_02000361"/>
        <obo:IAO_0000115>A municipality in Bahrain in the north central part of the country.</obo:IAO_0000115>
        <oboInOwl:hasOBONamespace>GAZ</oboInOwl:hasOBONamespace>
        <oboInOwl:id>GAZ:00078685</oboInOwl:id>
        <rdfs:label>Municipality of Madinat &apos;Isa</rdfs:label>
    </owl:NamedIndividual>
    


    <!-- http://purl.obolibrary.org/obo/GAZ_00089893 -->

    <owl:NamedIndividual rdf:about="http://purl.obolibrary.org/obo/GAZ_00089893">
        <obo:RO_0001025 rdf:resource="http://purl.obolibrary.org/obo/GAZ_00018504"/>
        <obo:IAO_0000115>A protected area including mangrove forests on the southern coast of Iran, particularly on and near the island of Qeshm in the Persian Gulf.</obo:IAO_0000115>
        <oboInOwl:hasOBONamespace>GAZ</oboInOwl:hasOBONamespace>
        <oboInOwl:id>GAZ:00089893</oboInOwl:id>
        <rdfs:label>Hara Protected Area</rdfs:label>
    </owl:NamedIndividual>
    


    <!-- http://purl.obolibrary.org/obo/GAZ_00124888 -->

    <owl:NamedIndividual rdf:about="http://purl.obolibrary.org/obo/GAZ_00124888">
        <obo:RO_0001025 rdf:resource="http://purl.obolibrary.org/obo/GAZ_00005295"/>
        <obo:IAO_0000115>A bay in the east of Bahrain, between Bahrain Island and Sitra island. The body of water is directly south of the Manama peninsula. The island of Nabih Saleh lies in the bay. A Ramsar Site.</obo:IAO_0000115>
        <oboInOwl:hasOBONamespace>GAZ</oboInOwl:hasOBONamespace>
        <oboInOwl:id>GAZ:00124888</oboInOwl:id>
        <rdfs:label>Tubli Bay</rdfs:label>
    </owl:NamedIndividual>
    


    <!-- http://purl.obolibrary.org/obo/GAZ_00145310 -->

    <owl:NamedIndividual rdf:about="http://purl.obolibrary.org/obo/GAZ_00145310">
        <obo:RO_0001025 rdf:resource="http://purl.obolibrary.org/obo/GAZ_00005295"/>
        <obo:IAO_0000115>An inlet of the Persian Gulf on the east coast of Saudi Arabia, separated from the main body of water by the peninsula of Qatar. It surrounds the islands of Bahrain.</obo:IAO_0000115>
        <oboInOwl:hasOBONamespace>GAZ</oboInOwl:hasOBONamespace>
        <oboInOwl:id>GAZ:00145310</oboInOwl:id>
        <rdfs:label>Gulf of Bahrain</rdfs:label>
    </owl:NamedIndividual>
    


    <!-- http://purl.obolibrary.org/obo/GAZ_00145498 -->

    <owl:NamedIndividual rdf:about="http://purl.obolibrary.org/obo/GAZ_00145498">
        <obo:RO_0001025 rdf:resource="http://purl.obolibrary.org/obo/GAZ_00005295"/>
        <obo:IAO_0000115>A saltwater creek located in Dubai, United Arab Emirates.</obo:IAO_0000115>
        <oboInOwl:hasOBONamespace>GAZ</oboInOwl:hasOBONamespace>
        <oboInOwl:id>GAZ:00145498</oboInOwl:id>
        <rdfs:label>Dubai Creek</rdfs:label>
    </owl:NamedIndividual>
    


    <!-- http://purl.obolibrary.org/obo/GAZ_00146397 -->

    <owl:NamedIndividual rdf:about="http://purl.obolibrary.org/obo/GAZ_00146397">
        <obo:RO_0001025 rdf:resource="http://purl.obolibrary.org/obo/GAZ_00005295"/>
        <obo:IAO_0000115>A bay in Umm al Quwain.</obo:IAO_0000115>
        <oboInOwl:hasOBONamespace>GAZ</oboInOwl:hasOBONamespace>
        <oboInOwl:id>GAZ:00146397</oboInOwl:id>
        <rdfs:label>Khawr al Baydah</rdfs:label>
    </owl:NamedIndividual>
    


    <!-- http://purl.obolibrary.org/obo/GAZ_00148786 -->

    <owl:NamedIndividual rdf:about="http://purl.obolibrary.org/obo/GAZ_00148786">
        <obo:IAO_0000115>A river on the central plateau of Iran, Isfahan Province. The Zayandeh starts in the Zagros Mountains and flows 400 km eastward before ending in the Gavkhouni swamp, a seasonal salt lake, southeast of Esfahan city.</obo:IAO_0000115>
        <oboInOwl:hasOBONamespace>GAZ</oboInOwl:hasOBONamespace>
        <oboInOwl:id>GAZ:00148786</oboInOwl:id>
        <rdfs:label>Zayandeh River</rdfs:label>
    </owl:NamedIndividual>
    


    <!-- http://purl.obolibrary.org/obo/GAZ_00148787 -->

    <owl:NamedIndividual rdf:about="http://purl.obolibrary.org/obo/GAZ_00148787">
        <obo:RO_0001025 rdf:resource="http://purl.obolibrary.org/obo/GAZ_00148786"/>
        <obo:IAO_0000115>A reservoir impounded by the Zayandeh Dam. Constructed 1972.</obo:IAO_0000115>
        <oboInOwl:hasOBONamespace>GAZ</oboInOwl:hasOBONamespace>
        <oboInOwl:id>GAZ:00148787</oboInOwl:id>
        <rdfs:label>Chadegan Reservoir</rdfs:label>
    </owl:NamedIndividual>
    


    <!-- http://purl.obolibrary.org/obo/GAZ_00148788 -->

    <owl:NamedIndividual rdf:about="http://purl.obolibrary.org/obo/GAZ_00148788">
        <obo:RO_0001025 rdf:resource="http://purl.obolibrary.org/obo/GAZ_00148786"/>
        <obo:IAO_0000115>A dam on the Zayandeh River impounding Chadegan Reservoir. Constructed 1972.</obo:IAO_0000115>
        <oboInOwl:hasOBONamespace>GAZ</oboInOwl:hasOBONamespace>
        <oboInOwl:id>GAZ:00148788</oboInOwl:id>
        <rdfs:label>Zayandeh Dam</rdfs:label>
    </owl:NamedIndividual>
    


    <!-- http://purl.obolibrary.org/obo/GAZ_00148789 -->

    <owl:NamedIndividual rdf:about="http://purl.obolibrary.org/obo/GAZ_00148789">
        <obo:IAO_0000115>A river.</obo:IAO_0000115>
        <oboInOwl:hasOBONamespace>GAZ</oboInOwl:hasOBONamespace>
        <oboInOwl:id>GAZ:00148789</oboInOwl:id>
        <rdfs:label>Dez River</rdfs:label>
    </owl:NamedIndividual>
    


    <!-- http://purl.obolibrary.org/obo/GAZ_00148790 -->

    <owl:NamedIndividual rdf:about="http://purl.obolibrary.org/obo/GAZ_00148790">
        <obo:RO_0001025 rdf:resource="http://purl.obolibrary.org/obo/GAZ_00148789"/>
        <obo:IAO_0000115>A dam and associated reservoir. Located on the Dez River in the southwestern foothills of the Zagros Mountains, about 15 km northeast of the city of Dezful, Khuzestan. Constructed 1963.</obo:IAO_0000115>
        <oboInOwl:hasOBONamespace>GAZ</oboInOwl:hasOBONamespace>
        <oboInOwl:id>GAZ:00148790</oboInOwl:id>
        <rdfs:label>Dez Dam</rdfs:label>
    </owl:NamedIndividual>
    


    <!-- http://purl.obolibrary.org/obo/GAZ_00148792 -->

    <owl:NamedIndividual rdf:about="http://purl.obolibrary.org/obo/GAZ_00148792">
        <obo:IAO_0000115>A hydroelectric dam on the Karun river in the province of Khuzestan.</obo:IAO_0000115>
        <oboInOwl:hasOBONamespace>GAZ</oboInOwl:hasOBONamespace>
        <oboInOwl:id>GAZ:00148792</oboInOwl:id>
        <rdfs:label>Karun-3 Dam</rdfs:label>
    </owl:NamedIndividual>
    


    <!-- http://purl.obolibrary.org/obo/GAZ_00148793 -->

    <owl:NamedIndividual rdf:about="http://purl.obolibrary.org/obo/GAZ_00148793">
        <obo:IAO_0000115>A hydroelectric dam under construction on the Karun river in the province of Chaharmahal and Bakhtiari, Iran.</obo:IAO_0000115>
        <oboInOwl:hasOBONamespace>GAZ</oboInOwl:hasOBONamespace>
        <oboInOwl:id>GAZ:00148793</oboInOwl:id>
        <rdfs:label>Karun-4 Dam</rdfs:label>
    </owl:NamedIndividual>
    


    <!-- http://purl.obolibrary.org/obo/GAZ_00148794 -->

    <owl:NamedIndividual rdf:about="http://purl.obolibrary.org/obo/GAZ_00148794">
        <obo:IAO_0000115>A hydroelectric dam on the Karun river in the province of Khuzestan, Iran. Completed 1976.</obo:IAO_0000115>
        <oboInOwl:hasOBONamespace>GAZ</oboInOwl:hasOBONamespace>
        <oboInOwl:id>GAZ:00148794</oboInOwl:id>
        <rdfs:label>Shahid Abbaspour Dam</rdfs:label>
    </owl:NamedIndividual>
    


    <!-- http://purl.obolibrary.org/obo/GAZ_00193960 -->

    <owl:NamedIndividual rdf:about="http://purl.obolibrary.org/obo/GAZ_00193960">
        <obo:IAO_0000115>A zoned rock-fill dam with a central core on the Euphrates River on the border of Adiyaman Province and Sanliurfa Province in Southeastern Anatolia Region of Turkey. Impounds Ataturk Baraj Golu.</obo:IAO_0000115>
        <oboInOwl:hasOBONamespace>GAZ</oboInOwl:hasOBONamespace>
        <oboInOwl:id>GAZ:00193960</oboInOwl:id>
        <rdfs:label>Ataturk Dam</rdfs:label>
    </owl:NamedIndividual>
    


    <!-- http://purl.obolibrary.org/obo/GAZ_00193961 -->

    <owl:NamedIndividual rdf:about="http://purl.obolibrary.org/obo/GAZ_00193961">
        <obo:IAO_0000115>A reservoir impounded by the Ataturk Dam.</obo:IAO_0000115>
        <oboInOwl:hasOBONamespace>GAZ</oboInOwl:hasOBONamespace>
        <oboInOwl:id>GAZ:00193961</oboInOwl:id>
        <rdfs:label>Ataturk Baraj Golu</rdfs:label>
    </owl:NamedIndividual>
    


    <!-- http://purl.obolibrary.org/obo/GAZ_00193962 -->

    <owl:NamedIndividual rdf:about="http://purl.obolibrary.org/obo/GAZ_00193962">
        <obo:IAO_0000115>A large complex of wetlands in Iraq that were part of the Tigris-Euphrates river system, along with the Huwaizah and Central Marshes. They almost totally destroyed during the 1990s by drainage projects, and have only recently seen some recovery.</obo:IAO_0000115>
        <oboInOwl:hasOBONamespace>GAZ</oboInOwl:hasOBONamespace>
        <oboInOwl:id>GAZ:00193962</oboInOwl:id>
        <rdfs:label>Haur Al Hammar</rdfs:label>
    </owl:NamedIndividual>
    


    <!-- http://purl.obolibrary.org/obo/GAZ_00193963 -->

    <owl:NamedIndividual rdf:about="http://purl.obolibrary.org/obo/GAZ_00193963">
        <obo:IAO_0000115>A large complex of wetlands in Iraq that were part of the Tigris-Euphrates river system, along with the Huwaizah and Hammar Marshes. They were almost completely desiccated following the 1991 uprisings in Iraq and have only in recent years started to show some signs of recovery. They stretched between Nasiriyah, Al-&apos;Uzair (Ezra&apos;s Tomb) and Al-Qurnah and were mainly fed by the Tigris and its distributaries.</obo:IAO_0000115>
        <oboInOwl:hasOBONamespace>GAZ</oboInOwl:hasOBONamespace>
        <oboInOwl:id>GAZ:00193963</oboInOwl:id>
        <rdfs:label>Qurna Marshes</rdfs:label>
    </owl:NamedIndividual>
    


    <!-- http://purl.obolibrary.org/obo/GAZ_00193964 -->

    <owl:NamedIndividual rdf:about="http://purl.obolibrary.org/obo/GAZ_00193964">
        <obo:IAO_0000115>A complex of marshes that straddle the Iraq and Iran border. The marshes are fed by the Tigris River in Iraq and Karkheh River in Iran.</obo:IAO_0000115>
        <oboInOwl:hasOBONamespace>GAZ</oboInOwl:hasOBONamespace>
        <oboInOwl:id>GAZ:00193964</oboInOwl:id>
        <rdfs:label>Haur Al Hawizeh</rdfs:label>
    </owl:NamedIndividual>
    


    <!-- http://purl.obolibrary.org/obo/GAZ_00193965 -->

    <owl:NamedIndividual rdf:about="http://purl.obolibrary.org/obo/GAZ_00193965">
        <obo:IAO_0000115>A dam located in the Elazig Province of Turkey. Constructed 1965-1975.</obo:IAO_0000115>
        <oboInOwl:hasOBONamespace>GAZ</oboInOwl:hasOBONamespace>
        <oboInOwl:id>GAZ:00193965</oboInOwl:id>
        <rdfs:label>Keban Dam</rdfs:label>
    </owl:NamedIndividual>
    


    <!-- http://purl.obolibrary.org/obo/GAZ_00193987 -->

    <owl:NamedIndividual rdf:about="http://purl.obolibrary.org/obo/GAZ_00193987">
        <obo:IAO_0000115>A drainage canal. This canal is 560 km in length/ It runs southeast from Al Mahmudiya near Baghdad down the right bank of the Shatt Al Gharraf and crosses the Euphrates just east of Nasiriya, burrowing beneath the riverbed in three large pipes. It then skirts round the southwestern edge of Haur Al Hammar, crosses the southeast corner of the haur (between raised embankments), and finally joins up with the man-made Shatt Al Basrah canal which links the southeast corner of Haur Al Hammar to the head of the Gulf via Khawr Al Zubair. Constructed 1950s-to-1992-12.</obo:IAO_0000115>
        <oboInOwl:hasOBONamespace>GAZ</oboInOwl:hasOBONamespace>
        <oboInOwl:id>GAZ:00193987</oboInOwl:id>
        <rdfs:label>Main Outfall Drain</rdfs:label>
    </owl:NamedIndividual>
    


    <!-- http://purl.obolibrary.org/obo/GAZ_00246729 -->

    <owl:NamedIndividual rdf:about="http://purl.obolibrary.org/obo/GAZ_00246729">
        <obo:RO_0001025 rdf:resource="http://purl.obolibrary.org/obo/GAZ_00006937"/>
        <obo:IAO_0000115>A bay. Located at the northeast corner of the main island of Bahrain, almost surrounded by the capital city Manama.</obo:IAO_0000115>
        <oboInOwl:hasOBONamespace>GAZ</oboInOwl:hasOBONamespace>
        <oboInOwl:id>GAZ:00246729</oboInOwl:id>
        <rdfs:label>Tubli Bay</rdfs:label>
    </owl:NamedIndividual>
    


    <!-- http://purl.obolibrary.org/obo/GAZ_00246730 -->

    <owl:NamedIndividual rdf:about="http://purl.obolibrary.org/obo/GAZ_00246730">
        <obo:RO_0001025 rdf:resource="http://purl.obolibrary.org/obo/GAZ_00006937"/>
        <obo:IAO_0000115>An artificial lake. Located in the north-central part of the main island of Bahrain. It was created by the excavation of sand from a large pit, and is fed by seepage from underground sources and by run-off from adjacent irrigated land.</obo:IAO_0000115>
        <oboInOwl:hasOBONamespace>GAZ</oboInOwl:hasOBONamespace>
        <oboInOwl:id>GAZ:00246730</oboInOwl:id>
        <rdfs:label>Lawzi Lake</rdfs:label>
    </owl:NamedIndividual>
    


    <!-- http://purl.obolibrary.org/obo/GAZ_00246731 -->

    <owl:NamedIndividual rdf:about="http://purl.obolibrary.org/obo/GAZ_00246731">
        <obo:RO_0001025 rdf:resource="http://purl.obolibrary.org/obo/GAZ_00006937"/>
        <obo:IAO_0000115>A protected area on the SW coast of Bahrain. The site comprises a long stretch of sheltered sandy beach backed by low sand dunes and an adjacent small area of inter-tidal mudflats and sand flats.</obo:IAO_0000115>
        <oboInOwl:hasOBONamespace>GAZ</oboInOwl:hasOBONamespace>
        <oboInOwl:id>GAZ:00246731</oboInOwl:id>
        <rdfs:label>Mumtalah</rdfs:label>
    </owl:NamedIndividual>
    


    <!-- http://purl.obolibrary.org/obo/GAZ_00246732 -->

    <owl:NamedIndividual rdf:about="http://purl.obolibrary.org/obo/GAZ_00246732">
        <obo:RO_0001025 rdf:resource="http://purl.obolibrary.org/obo/GAZ_00006937"/>
        <obo:IAO_0000115>A large area of relatively undisturbed inter-tidal mudflats located on the SE coast of Bahrain.</obo:IAO_0000115>
        <oboInOwl:hasOBONamespace>GAZ</oboInOwl:hasOBONamespace>
        <oboInOwl:id>GAZ:00246732</oboInOwl:id>
        <rdfs:label>Ras Hayan</rdfs:label>
    </owl:NamedIndividual>
    


    <!-- http://purl.obolibrary.org/obo/GAZ_00248023 -->

    <owl:NamedIndividual rdf:about="http://purl.obolibrary.org/obo/GAZ_00248023">
        <obo:RO_0001025 rdf:resource="http://purl.obolibrary.org/obo/GAZ_00005295"/>
        <obo:IAO_0000115>An island.</obo:IAO_0000115>
        <oboInOwl:hasOBONamespace>GAZ</oboInOwl:hasOBONamespace>
        <oboInOwl:id>GAZ:00248023</oboInOwl:id>
        <rdfs:label>Sir Bani Yas</rdfs:label>
    </owl:NamedIndividual>
    


    <!-- http://purl.obolibrary.org/obo/GAZ_00248024 -->

    <owl:NamedIndividual rdf:about="http://purl.obolibrary.org/obo/GAZ_00248024">
        <obo:RO_0001025 rdf:resource="http://purl.obolibrary.org/obo/GAZ_00005295"/>
        <obo:IAO_0000115>A channel.</obo:IAO_0000115>
        <oboInOwl:hasOBONamespace>GAZ</oboInOwl:hasOBONamespace>
        <oboInOwl:id>GAZ:00248024</oboInOwl:id>
        <rdfs:label>Khawr al Bazm</rdfs:label>
    </owl:NamedIndividual>
    


    <!-- http://purl.obolibrary.org/obo/GAZ_00248025 -->

    <owl:NamedIndividual rdf:about="http://purl.obolibrary.org/obo/GAZ_00248025">
        <obo:RO_0001025 rdf:resource="http://purl.obolibrary.org/obo/GAZ_00005295"/>
        <obo:IAO_0000115>An island.</obo:IAO_0000115>
        <oboInOwl:hasOBONamespace>GAZ</oboInOwl:hasOBONamespace>
        <oboInOwl:id>GAZ:00248025</oboInOwl:id>
        <rdfs:label>Bu Khushayshah</rdfs:label>
    </owl:NamedIndividual>
    


    <!-- http://purl.obolibrary.org/obo/GAZ_00248026 -->

    <owl:NamedIndividual rdf:about="http://purl.obolibrary.org/obo/GAZ_00248026">
        <obo:RO_0001025 rdf:resource="http://purl.obolibrary.org/obo/GAZ_00005295"/>
        <obo:IAO_0000115>An island.</obo:IAO_0000115>
        <oboInOwl:hasOBONamespace>GAZ</oboInOwl:hasOBONamespace>
        <oboInOwl:id>GAZ:00248026</oboInOwl:id>
        <rdfs:label>Al Futaysi</rdfs:label>
    </owl:NamedIndividual>
    


    <!-- http://purl.obolibrary.org/obo/GAZ_00248027 -->

    <owl:NamedIndividual rdf:about="http://purl.obolibrary.org/obo/GAZ_00248027">
        <obo:RO_0001025 rdf:resource="http://purl.obolibrary.org/obo/GAZ_00005295"/>
        <obo:IAO_0000115>An island.</obo:IAO_0000115>
        <oboInOwl:hasOBONamespace>GAZ</oboInOwl:hasOBONamespace>
        <oboInOwl:id>GAZ:00248027</oboInOwl:id>
        <rdfs:label>Halat al Bahrani</rdfs:label>
    </owl:NamedIndividual>
    


    <!-- http://purl.obolibrary.org/obo/GAZ_00248028 -->

    <owl:NamedIndividual rdf:about="http://purl.obolibrary.org/obo/GAZ_00248028">
        <obo:RO_0001025 rdf:resource="http://purl.obolibrary.org/obo/GAZ_00005295"/>
        <obo:IAO_0000115>An island.</obo:IAO_0000115>
        <oboInOwl:hasOBONamespace>GAZ</oboInOwl:hasOBONamespace>
        <oboInOwl:id>GAZ:00248028</oboInOwl:id>
        <rdfs:label>&apos;Ushsh</rdfs:label>
    </owl:NamedIndividual>
    


    <!-- http://purl.obolibrary.org/obo/GAZ_00248029 -->

    <owl:NamedIndividual rdf:about="http://purl.obolibrary.org/obo/GAZ_00248029">
        <obo:RO_0001025 rdf:resource="http://purl.obolibrary.org/obo/GAZ_00005295"/>
        <obo:IAO_0000115>An island.</obo:IAO_0000115>
        <oboInOwl:hasOBONamespace>GAZ</oboInOwl:hasOBONamespace>
        <oboInOwl:id>GAZ:00248029</oboInOwl:id>
        <rdfs:label>Umm &apos;Amim</rdfs:label>
    </owl:NamedIndividual>
    


    <!-- http://purl.obolibrary.org/obo/GAZ_00248030 -->

    <owl:NamedIndividual rdf:about="http://purl.obolibrary.org/obo/GAZ_00248030">
        <obo:RO_0001025 rdf:resource="http://purl.obolibrary.org/obo/GAZ_00005295"/>
        <obo:IAO_0000115>An island.</obo:IAO_0000115>
        <oboInOwl:hasOBONamespace>GAZ</oboInOwl:hasOBONamespace>
        <oboInOwl:id>GAZ:00248030</oboInOwl:id>
        <rdfs:label>Jananah</rdfs:label>
    </owl:NamedIndividual>
    


    <!-- http://purl.obolibrary.org/obo/GAZ_00248031 -->

    <owl:NamedIndividual rdf:about="http://purl.obolibrary.org/obo/GAZ_00248031">
        <rdf:type rdf:resource="http://purl.obolibrary.org/obo/ENVO_00000167"/>
        <obo:RO_0001025 rdf:resource="http://purl.obolibrary.org/obo/GAZ_00005295"/>
        <obo:IAO_0000115>A shoal.</obo:IAO_0000115>
        <oboInOwl:hasOBONamespace>GAZ</oboInOwl:hasOBONamespace>
        <oboInOwl:id>GAZ:00248031</oboInOwl:id>
        <rdfs:label>Bu Tinah</rdfs:label>
    </owl:NamedIndividual>
    


    <!-- http://purl.obolibrary.org/obo/GAZ_00248035 -->

    <owl:NamedIndividual rdf:about="http://purl.obolibrary.org/obo/GAZ_00248035">
        <obo:RO_0001025 rdf:resource="http://purl.obolibrary.org/obo/GAZ_00005295"/>
        <obo:IAO_0000115>An island. A satellite of Sir Bani Yas.</obo:IAO_0000115>
        <oboInOwl:hasOBONamespace>GAZ</oboInOwl:hasOBONamespace>
        <oboInOwl:id>GAZ:00248035</oboInOwl:id>
        <rdfs:label>Umm Qassar</rdfs:label>
    </owl:NamedIndividual>
    


    <!-- http://purl.obolibrary.org/obo/GAZ_00248036 -->

    <owl:NamedIndividual rdf:about="http://purl.obolibrary.org/obo/GAZ_00248036">
        <obo:RO_0001025 rdf:resource="http://purl.obolibrary.org/obo/GAZ_00005295"/>
        <oboInOwl:hasOBONamespace>GAZ</oboInOwl:hasOBONamespace>
        <oboInOwl:id>GAZ:00248036</oboInOwl:id>
        <rdfs:label>Umm al Kirkum</rdfs:label>
    </owl:NamedIndividual>
    


    <!-- http://purl.obolibrary.org/obo/GAZ_00248037 -->

    <owl:NamedIndividual rdf:about="http://purl.obolibrary.org/obo/GAZ_00248037">
        <obo:RO_0001025 rdf:resource="http://purl.obolibrary.org/obo/GAZ_00005295"/>
        <oboInOwl:hasOBONamespace>GAZ</oboInOwl:hasOBONamespace>
        <oboInOwl:id>GAZ:00248037</oboInOwl:id>
        <rdfs:label>Ghasha</rdfs:label>
    </owl:NamedIndividual>
    


    <!-- http://purl.obolibrary.org/obo/GAZ_00248038 -->

    <owl:NamedIndividual rdf:about="http://purl.obolibrary.org/obo/GAZ_00248038">
        <obo:RO_0001025 rdf:resource="http://purl.obolibrary.org/obo/GAZ_00005295"/>
        <obo:IAO_0000115>An island.</obo:IAO_0000115>
        <oboInOwl:hasOBONamespace>GAZ</oboInOwl:hasOBONamespace>
        <oboInOwl:id>GAZ:00248038</oboInOwl:id>
        <rdfs:label>Al Yasat</rdfs:label>
    </owl:NamedIndividual>
    


    <!-- http://purl.obolibrary.org/obo/GAZ_00248039 -->

    <owl:NamedIndividual rdf:about="http://purl.obolibrary.org/obo/GAZ_00248039">
        <obo:RO_0001025 rdf:resource="http://purl.obolibrary.org/obo/GAZ_00005295"/>
        <obo:IAO_0000115>An island.</obo:IAO_0000115>
        <oboInOwl:hasOBONamespace>GAZ</oboInOwl:hasOBONamespace>
        <oboInOwl:id>GAZ:00248039</oboInOwl:id>
        <rdfs:label>Al Yasat as Sufla</rdfs:label>
    </owl:NamedIndividual>
    


    <!-- http://purl.obolibrary.org/obo/GAZ_00248040 -->

    <owl:NamedIndividual rdf:about="http://purl.obolibrary.org/obo/GAZ_00248040">
        <obo:RO_0001025 rdf:resource="http://purl.obolibrary.org/obo/GAZ_00005295"/>
        <obo:IAO_0000115>An island.</obo:IAO_0000115>
        <oboInOwl:hasOBONamespace>GAZ</oboInOwl:hasOBONamespace>
        <oboInOwl:id>GAZ:00248040</oboInOwl:id>
        <rdfs:label>Al Yasat al &apos;Ulya</rdfs:label>
    </owl:NamedIndividual>
    


    <!-- http://purl.obolibrary.org/obo/GAZ_00248041 -->

    <owl:NamedIndividual rdf:about="http://purl.obolibrary.org/obo/GAZ_00248041">
        <obo:RO_0001025 rdf:resource="http://purl.obolibrary.org/obo/GAZ_00005295"/>
        <obo:IAO_0000115>An island.</obo:IAO_0000115>
        <oboInOwl:hasOBONamespace>GAZ</oboInOwl:hasOBONamespace>
        <oboInOwl:id>GAZ:00248041</oboInOwl:id>
        <rdfs:label>Ghaghah</rdfs:label>
    </owl:NamedIndividual>
    


    <!-- http://purl.obolibrary.org/obo/GAZ_00248042 -->

    <owl:NamedIndividual rdf:about="http://purl.obolibrary.org/obo/GAZ_00248042">
        <obo:RO_0001025 rdf:resource="http://purl.obolibrary.org/obo/GAZ_00005295"/>
        <obo:IAO_0000115>An island.</obo:IAO_0000115>
        <oboInOwl:hasOBONamespace>GAZ</oboInOwl:hasOBONamespace>
        <oboInOwl:id>GAZ:00248042</oboInOwl:id>
        <rdfs:label>Umm al Hatab</rdfs:label>
    </owl:NamedIndividual>
    


    <!-- http://purl.obolibrary.org/obo/GAZ_00248043 -->

    <owl:NamedIndividual rdf:about="http://purl.obolibrary.org/obo/GAZ_00248043">
        <obo:RO_0001025 rdf:resource="http://purl.obolibrary.org/obo/GAZ_00005295"/>
        <obo:IAO_0000115>An island.</obo:IAO_0000115>
        <oboInOwl:hasOBONamespace>GAZ</oboInOwl:hasOBONamespace>
        <oboInOwl:id>GAZ:00248043</oboInOwl:id>
        <rdfs:label>Makasib</rdfs:label>
    </owl:NamedIndividual>
    


    <!-- http://purl.obolibrary.org/obo/GAZ_00248044 -->

    <owl:NamedIndividual rdf:about="http://purl.obolibrary.org/obo/GAZ_00248044">
        <obo:RO_0001025 rdf:resource="http://purl.obolibrary.org/obo/GAZ_00005295"/>
        <obo:IAO_0000115>An island.</obo:IAO_0000115>
        <oboInOwl:hasOBONamespace>GAZ</oboInOwl:hasOBONamespace>
        <oboInOwl:id>GAZ:00248044</oboInOwl:id>
        <rdfs:label>Al Qaffay</rdfs:label>
    </owl:NamedIndividual>
    


    <!-- http://purl.obolibrary.org/obo/GAZ_00248045 -->

    <owl:NamedIndividual rdf:about="http://purl.obolibrary.org/obo/GAZ_00248045">
        <obo:RO_0001025 rdf:resource="http://purl.obolibrary.org/obo/GAZ_00005295"/>
        <obo:IAO_0000115>An island.</obo:IAO_0000115>
        <oboInOwl:hasOBONamespace>GAZ</oboInOwl:hasOBONamespace>
        <oboInOwl:id>GAZ:00248045</oboInOwl:id>
        <rdfs:label>Muhammaliyah</rdfs:label>
    </owl:NamedIndividual>
    


    <!-- http://purl.obolibrary.org/obo/GAZ_00248046 -->

    <owl:NamedIndividual rdf:about="http://purl.obolibrary.org/obo/GAZ_00248046">
        <obo:RO_0001025 rdf:resource="http://purl.obolibrary.org/obo/GAZ_00005295"/>
        <obo:IAO_0000115>An offshore island.</obo:IAO_0000115>
        <oboInOwl:hasOBONamespace>GAZ</oboInOwl:hasOBONamespace>
        <oboInOwl:id>GAZ:00248046</oboInOwl:id>
        <rdfs:label>Dayyinah</rdfs:label>
    </owl:NamedIndividual>
    


    <!-- http://purl.obolibrary.org/obo/GAZ_00248047 -->

    <owl:NamedIndividual rdf:about="http://purl.obolibrary.org/obo/GAZ_00248047">
        <obo:RO_0001025 rdf:resource="http://purl.obolibrary.org/obo/GAZ_00005295"/>
        <obo:IAO_0000115>An offshore island.</obo:IAO_0000115>
        <oboInOwl:hasOBONamespace>GAZ</oboInOwl:hasOBONamespace>
        <oboInOwl:id>GAZ:00248047</oboInOwl:id>
        <rdfs:label>Qarnayn</rdfs:label>
    </owl:NamedIndividual>
    


    <!-- http://purl.obolibrary.org/obo/GAZ_00248048 -->

    <owl:NamedIndividual rdf:about="http://purl.obolibrary.org/obo/GAZ_00248048">
        <obo:RO_0001025 rdf:resource="http://purl.obolibrary.org/obo/GAZ_00005295"/>
        <obo:IAO_0000115>An offshore island.</obo:IAO_0000115>
        <oboInOwl:hasOBONamespace>GAZ</oboInOwl:hasOBONamespace>
        <oboInOwl:id>GAZ:00248048</oboInOwl:id>
        <rdfs:label>Arzanah</rdfs:label>
    </owl:NamedIndividual>
    


    <!-- http://purl.obolibrary.org/obo/GAZ_00248049 -->

    <owl:NamedIndividual rdf:about="http://purl.obolibrary.org/obo/GAZ_00248049">
        <obo:RO_0001025 rdf:resource="http://purl.obolibrary.org/obo/GAZ_00005295"/>
        <obo:IAO_0000115>An offshore island.</obo:IAO_0000115>
        <oboInOwl:hasOBONamespace>GAZ</oboInOwl:hasOBONamespace>
        <oboInOwl:id>GAZ:00248049</oboInOwl:id>
        <rdfs:label>Zirkuh</rdfs:label>
    </owl:NamedIndividual>
    


    <!-- http://purl.obolibrary.org/obo/GAZ_00248050 -->

    <owl:NamedIndividual rdf:about="http://purl.obolibrary.org/obo/GAZ_00248050">
        <obo:RO_0001025 rdf:resource="http://purl.obolibrary.org/obo/GAZ_00005295"/>
        <obo:IAO_0000115>An island off eastern Abu Dhabi.</obo:IAO_0000115>
        <oboInOwl:hasOBONamespace>GAZ</oboInOwl:hasOBONamespace>
        <oboInOwl:id>GAZ:00248050</oboInOwl:id>
        <rdfs:label>As Sa&apos;diyat</rdfs:label>
    </owl:NamedIndividual>
    


    <!-- http://purl.obolibrary.org/obo/GAZ_00248051 -->

    <owl:NamedIndividual rdf:about="http://purl.obolibrary.org/obo/GAZ_00248051">
        <obo:RO_0001025 rdf:resource="http://purl.obolibrary.org/obo/GAZ_00005295"/>
        <obo:IAO_0000115>An island off eastern Abu Dhabi.</obo:IAO_0000115>
        <oboInOwl:hasOBONamespace>GAZ</oboInOwl:hasOBONamespace>
        <oboInOwl:id>GAZ:00248051</oboInOwl:id>
        <rdfs:label>Jazirat Ramhan</rdfs:label>
    </owl:NamedIndividual>
    


    <!-- http://purl.obolibrary.org/obo/GAZ_00248052 -->

    <owl:NamedIndividual rdf:about="http://purl.obolibrary.org/obo/GAZ_00248052">
        <obo:RO_0001025 rdf:resource="http://purl.obolibrary.org/obo/GAZ_00005295"/>
        <obo:IAO_0000115>An island off eastern Abu Dhabi.</obo:IAO_0000115>
        <oboInOwl:hasOBONamespace>GAZ</oboInOwl:hasOBONamespace>
        <oboInOwl:id>GAZ:00248052</oboInOwl:id>
        <rdfs:label>Bu Hayl</rdfs:label>
    </owl:NamedIndividual>
    


    <!-- http://purl.obolibrary.org/obo/GAZ_00248053 -->

    <owl:NamedIndividual rdf:about="http://purl.obolibrary.org/obo/GAZ_00248053">
        <obo:RO_0001025 rdf:resource="http://purl.obolibrary.org/obo/GAZ_00005295"/>
        <obo:IAO_0000115>An island off eastern Abu Dhabi.</obo:IAO_0000115>
        <oboInOwl:hasOBONamespace>GAZ</oboInOwl:hasOBONamespace>
        <oboInOwl:id>GAZ:00248053</oboInOwl:id>
        <rdfs:label>Hayl</rdfs:label>
    </owl:NamedIndividual>
    


    <!-- http://purl.obolibrary.org/obo/GAZ_00248054 -->

    <owl:NamedIndividual rdf:about="http://purl.obolibrary.org/obo/GAZ_00248054">
        <obo:RO_0001025 rdf:resource="http://purl.obolibrary.org/obo/GAZ_00005295"/>
        <obo:IAO_0000115>An island off eastern Abu Dhabi.</obo:IAO_0000115>
        <oboInOwl:hasOBONamespace>GAZ</oboInOwl:hasOBONamespace>
        <oboInOwl:id>GAZ:00248054</oboInOwl:id>
        <rdfs:label>Jazirat Ra&apos;s Ghurab</rdfs:label>
    </owl:NamedIndividual>
    


    <!-- http://purl.obolibrary.org/obo/GAZ_00248055 -->

    <owl:NamedIndividual rdf:about="http://purl.obolibrary.org/obo/GAZ_00248055">
        <obo:RO_0001025 rdf:resource="http://purl.obolibrary.org/obo/GAZ_00005295"/>
        <obo:IAO_0000115>An island off eastern Abu Dhabi.</obo:IAO_0000115>
        <oboInOwl:hasOBONamespace>GAZ</oboInOwl:hasOBONamespace>
        <oboInOwl:id>GAZ:00248055</oboInOwl:id>
        <rdfs:label>Ra&apos;s Ghanadah</rdfs:label>
    </owl:NamedIndividual>
    


    <!-- http://purl.obolibrary.org/obo/GAZ_00248057 -->

    <owl:NamedIndividual rdf:about="http://purl.obolibrary.org/obo/GAZ_00248057">
        <obo:RO_0001025 rdf:resource="http://purl.obolibrary.org/obo/GAZ_00005295"/>
        <obo:IAO_0000115>An island. Located in the Persian Gulf, 75 km from the mainland coast of Abu Dhabi, Abu Dhabi Emirate.</obo:IAO_0000115>
        <oboInOwl:hasOBONamespace>GAZ</oboInOwl:hasOBONamespace>
        <oboInOwl:id>GAZ:00248057</oboInOwl:id>
        <rdfs:label>Sir Bu Nu&apos;ayr</rdfs:label>
    </owl:NamedIndividual>
    


    <!-- http://purl.obolibrary.org/obo/GAZ_00248061 -->

    <owl:NamedIndividual rdf:about="http://purl.obolibrary.org/obo/GAZ_00248061">
        <rdf:type rdf:resource="http://purl.obolibrary.org/obo/ENVO_00000475"/>
        <obo:RO_0001025 rdf:resource="http://purl.obolibrary.org/obo/GAZ_00005295"/>
        <obo:IAO_0000115>A tidal creek. An arm of Khor Zawra.</obo:IAO_0000115>
        <oboInOwl:hasOBONamespace>GAZ</oboInOwl:hasOBONamespace>
        <oboInOwl:id>GAZ:00248061</oboInOwl:id>
        <rdfs:label>Khor Zawra</rdfs:label>
    </owl:NamedIndividual>
    


    <!-- http://purl.obolibrary.org/obo/GAZ_00248062 -->

    <owl:NamedIndividual rdf:about="http://purl.obolibrary.org/obo/GAZ_00248062">
        <obo:RO_0001025 rdf:resource="http://purl.obolibrary.org/obo/GAZ_00005295"/>
        <obo:IAO_0000115>A wetland located on the Arabian Gulf coast east of Umm al Qaiwain city and on the landward (southeast) side of Sinaiya Island, Umm al Qaiwain Emirate. It comprises a vast complex of lagoons, 20 km long by an average of 4 km wide, with about 25 low sandy islands, each of less than 50 ha in extent except for the three mangrove-covered round islands of Jazirat al Ghubbah (Ghallah), which are between one and two km in diameter.</obo:IAO_0000115>
        <oboInOwl:hasOBONamespace>GAZ</oboInOwl:hasOBONamespace>
        <oboInOwl:id>GAZ:00248062</oboInOwl:id>
        <rdfs:label>Khor al Beidah</rdfs:label>
    </owl:NamedIndividual>
    


    <!-- http://purl.obolibrary.org/obo/GAZ_00248063 -->

    <owl:NamedIndividual rdf:about="http://purl.obolibrary.org/obo/GAZ_00248063">
        <obo:RO_0001025 rdf:resource="http://purl.obolibrary.org/obo/GAZ_00005295"/>
        <obo:IAO_0000115>An island.</obo:IAO_0000115>
        <oboInOwl:hasOBONamespace>GAZ</oboInOwl:hasOBONamespace>
        <oboInOwl:id>GAZ:00248063</oboInOwl:id>
        <rdfs:label>Jazirat as Siniyah</rdfs:label>
    </owl:NamedIndividual>
    


    <!-- http://purl.obolibrary.org/obo/GAZ_00248064 -->

    <owl:NamedIndividual rdf:about="http://purl.obolibrary.org/obo/GAZ_00248064">
        <obo:RO_0001025 rdf:resource="http://purl.obolibrary.org/obo/GAZ_00005295"/>
        <obo:IAO_0000115>An island.</obo:IAO_0000115>
        <oboInOwl:hasOBONamespace>GAZ</oboInOwl:hasOBONamespace>
        <oboInOwl:id>GAZ:00248064</oboInOwl:id>
        <rdfs:label>Jazirat al Ghallah</rdfs:label>
    </owl:NamedIndividual>
    


    <!-- http://purl.obolibrary.org/obo/GAZ_00248065 -->

    <owl:NamedIndividual rdf:about="http://purl.obolibrary.org/obo/GAZ_00248065">
        <obo:RO_0001025 rdf:resource="http://purl.obolibrary.org/obo/GAZ_00248062"/>
        <obo:IAO_0000115>Three mangrove-covered islands.</obo:IAO_0000115>
        <oboInOwl:hasOBONamespace>GAZ</oboInOwl:hasOBONamespace>
        <oboInOwl:id>GAZ:00248065</oboInOwl:id>
        <rdfs:label>Jazirat al Ghubbah</rdfs:label>
    </owl:NamedIndividual>
    


    <!-- http://purl.obolibrary.org/obo/GAZ_00248066 -->

    <owl:NamedIndividual rdf:about="http://purl.obolibrary.org/obo/GAZ_00248066">
        <obo:RO_0001025 rdf:resource="http://purl.obolibrary.org/obo/GAZ_00248062"/>
        <obo:IAO_0000115>The southwestern portion of the lagoons of Khor al Beidah.</obo:IAO_0000115>
        <oboInOwl:hasOBONamespace>GAZ</oboInOwl:hasOBONamespace>
        <oboInOwl:id>GAZ:00248066</oboInOwl:id>
        <rdfs:label>Khor Umm al Qaiwain</rdfs:label>
    </owl:NamedIndividual>
    


    <!-- http://purl.obolibrary.org/obo/GAZ_00248067 -->

    <owl:NamedIndividual rdf:about="http://purl.obolibrary.org/obo/GAZ_00248067">
        <obo:RO_0001025 rdf:resource="http://purl.obolibrary.org/obo/GAZ_00005295"/>
        <obo:IAO_0000115>A complex of shallow tidal lagoons and inter-tidal mudflats on the Gulf coast, with areas of higher ground covered with halophytic scrub.</obo:IAO_0000115>
        <oboInOwl:hasOBONamespace>GAZ</oboInOwl:hasOBONamespace>
        <oboInOwl:id>GAZ:00248067</oboInOwl:id>
        <rdfs:label>Al Jazeerah Khor</rdfs:label>
    </owl:NamedIndividual>
    


    <!-- http://purl.obolibrary.org/obo/GAZ_00248068 -->

    <owl:NamedIndividual rdf:about="http://purl.obolibrary.org/obo/GAZ_00248068">
        <obo:RO_0001025 rdf:resource="http://purl.obolibrary.org/obo/GAZ_00005295"/>
        <obo:IAO_0000115>An island. Off the W side of the Musandam Peninsula.</obo:IAO_0000115>
        <oboInOwl:hasOBONamespace>GAZ</oboInOwl:hasOBONamespace>
        <oboInOwl:id>GAZ:00248068</oboInOwl:id>
        <rdfs:label>Jazirat Hulaylah</rdfs:label>
    </owl:NamedIndividual>
    


    <!-- http://purl.obolibrary.org/obo/GAZ_00248069 -->

    <owl:NamedIndividual rdf:about="http://purl.obolibrary.org/obo/GAZ_00248069">
        <obo:RO_0001025 rdf:resource="http://purl.obolibrary.org/obo/GAZ_00005295"/>
        <obo:IAO_0000115>An island.</obo:IAO_0000115>
        <oboInOwl:hasOBONamespace>GAZ</oboInOwl:hasOBONamespace>
        <oboInOwl:id>GAZ:00248069</oboInOwl:id>
        <rdfs:label>Jazirat al Hamra&apos;</rdfs:label>
    </owl:NamedIndividual>
    


    <!-- http://purl.obolibrary.org/obo/GAZ_00248070 -->

    <owl:NamedIndividual rdf:about="http://purl.obolibrary.org/obo/GAZ_00248070">
        <obo:RO_0001025 rdf:resource="http://purl.obolibrary.org/obo/GAZ_00005295"/>
        <obo:IAO_0000115>An island.</obo:IAO_0000115>
        <oboInOwl:hasOBONamespace>GAZ</oboInOwl:hasOBONamespace>
        <oboInOwl:id>GAZ:00248070</oboInOwl:id>
        <rdfs:label>Jazirat Qurmah</rdfs:label>
    </owl:NamedIndividual>
    


    <!-- http://purl.obolibrary.org/obo/GAZ_00248071 -->

    <owl:NamedIndividual rdf:about="http://purl.obolibrary.org/obo/GAZ_00248071">
        <obo:RO_0001025 rdf:resource="http://purl.obolibrary.org/obo/GAZ_00005295"/>
        <obo:IAO_0000115>A bay on the east coast of the UAE in Fujairah and Sharjah Emirates, and straddling the border with Oman.</obo:IAO_0000115>
        <oboInOwl:hasOBONamespace>GAZ</oboInOwl:hasOBONamespace>
        <oboInOwl:id>GAZ:00248071</oboInOwl:id>
        <rdfs:label>Dawhat Diba</rdfs:label>
    </owl:NamedIndividual>
    


    <!-- http://purl.obolibrary.org/obo/GAZ_00248075 -->

    <owl:NamedIndividual rdf:about="http://purl.obolibrary.org/obo/GAZ_00248075">
        <obo:RO_0001025 rdf:resource="http://purl.obolibrary.org/obo/GAZ_00005295"/>
        <obo:IAO_0000115>A tidal inlet. Khor Kalba is a small, shallow, tidal inlet with ramifying channels formed by the outlet of Wadi Rumh.</obo:IAO_0000115>
        <oboInOwl:hasOBONamespace>GAZ</oboInOwl:hasOBONamespace>
        <oboInOwl:id>GAZ:00248075</oboInOwl:id>
        <rdfs:label>Khor Kalba</rdfs:label>
    </owl:NamedIndividual>
    


    <!-- http://purl.obolibrary.org/obo/GAZ_00250781 -->

    <owl:NamedIndividual rdf:about="http://purl.obolibrary.org/obo/GAZ_00250781">
        <obo:RO_0001025 rdf:resource="http://purl.obolibrary.org/obo/GAZ_00004481"/>
        <obo:IAO_0000115>A massif of the Central Iranian Plateau, Kerman province, Iran, an eastern outlier of the Zagros mountains.</obo:IAO_0000115>
        <oboInOwl:hasOBONamespace>GAZ</oboInOwl:hasOBONamespace>
        <oboInOwl:id>GAZ:00250781</oboInOwl:id>
        <rdfs:label>Hazaran Massif</rdfs:label>
    </owl:NamedIndividual>
    


    <!-- http://purl.obolibrary.org/obo/GAZ_00250786 -->

    <owl:NamedIndividual rdf:about="http://purl.obolibrary.org/obo/GAZ_00250786">
        <obo:IAO_0000115>A dam.</obo:IAO_0000115>
        <oboInOwl:hasOBONamespace>GAZ</oboInOwl:hasOBONamespace>
        <oboInOwl:id>GAZ:00250786</oboInOwl:id>
        <rdfs:label>Jiroft Dam</rdfs:label>
    </owl:NamedIndividual>
    


    <!-- http://purl.obolibrary.org/obo/GAZ_00250857 -->

    <owl:NamedIndividual rdf:about="http://purl.obolibrary.org/obo/GAZ_00250857">
        <obo:RO_0001025 rdf:resource="http://purl.obolibrary.org/obo/GAZ_00004481"/>
        <obo:IAO_0000115>A wetland. Located in a broad intermontane basin in the western Zagros Mountains about 20-30 km northwest of Kermanshah, Kermanshah Province.</obo:IAO_0000115>
        <oboInOwl:hasOBONamespace>GAZ</oboInOwl:hasOBONamespace>
        <oboInOwl:id>GAZ:00250857</oboInOwl:id>
        <rdfs:label>Hashelan Marsh</rdfs:label>
    </owl:NamedIndividual>
    


    <!-- http://purl.obolibrary.org/obo/GAZ_00250859 -->

    <owl:NamedIndividual rdf:about="http://purl.obolibrary.org/obo/GAZ_00250859">
        <obo:IAO_0000115>A river in Khuzestan Province. It rises in the Zagros Mountains, and passes north of Shush, eventually falling into the Tigris just below its confluence with the Euphrates very near to the Iran-Iraq border.</obo:IAO_0000115>
        <oboInOwl:hasOBONamespace>GAZ</oboInOwl:hasOBONamespace>
        <oboInOwl:id>GAZ:00250859</oboInOwl:id>
        <rdfs:label>Karkheh River</rdfs:label>
    </owl:NamedIndividual>
    


    <!-- http://purl.obolibrary.org/obo/GAZ_00250861 -->

    <owl:NamedIndividual rdf:about="http://purl.obolibrary.org/obo/GAZ_00250861">
        <obo:RO_0001025 rdf:resource="http://purl.obolibrary.org/obo/GAZ_00250859"/>
        <obo:IAO_0000115>A large multi-purpose earthen embankment dam built in Iran on the Karkheh River. Constructed 2001.</obo:IAO_0000115>
        <oboInOwl:hasOBONamespace>GAZ</oboInOwl:hasOBONamespace>
        <oboInOwl:id>GAZ:00250861</oboInOwl:id>
        <rdfs:label>Karkheh Dam</rdfs:label>
    </owl:NamedIndividual>
    


    <!-- http://purl.obolibrary.org/obo/GAZ_00250868 -->

    <owl:NamedIndividual rdf:about="http://purl.obolibrary.org/obo/GAZ_00250868">
        <obo:RO_0001025 rdf:resource="http://purl.obolibrary.org/obo/GAZ_00005295"/>
        <obo:IAO_0000115>A marine channel at the head of the Persian Gulf.</obo:IAO_0000115>
        <oboInOwl:hasOBONamespace>GAZ</oboInOwl:hasOBONamespace>
        <oboInOwl:id>GAZ:00250868</oboInOwl:id>
        <rdfs:label>Khor-al Amaya</rdfs:label>
    </owl:NamedIndividual>
    


    <!-- http://purl.obolibrary.org/obo/GAZ_00250869 -->

    <owl:NamedIndividual rdf:about="http://purl.obolibrary.org/obo/GAZ_00250869">
        <obo:RO_0001025 rdf:resource="http://purl.obolibrary.org/obo/GAZ_00005295"/>
        <obo:IAO_0000115>A marine channel at the head of the Persian Gulf.</obo:IAO_0000115>
        <oboInOwl:hasOBONamespace>GAZ</oboInOwl:hasOBONamespace>
        <oboInOwl:id>GAZ:00250869</oboInOwl:id>
        <rdfs:label>Khor Musa</rdfs:label>
    </owl:NamedIndividual>
    


    <!-- http://purl.obolibrary.org/obo/GAZ_00250872 -->

    <owl:NamedIndividual rdf:about="http://purl.obolibrary.org/obo/GAZ_00250872">
        <obo:RO_0001025 rdf:resource="http://purl.obolibrary.org/obo/GAZ_00004481"/>
        <obo:IAO_0000115>A wetland. A freshwater marsh. Located in the upper drainage of the Karun River in the Zagros Mountains, about 95 km west of Shahreza, Chaharmahal and Bakhtiari.</obo:IAO_0000115>
        <oboInOwl:hasOBONamespace>GAZ</oboInOwl:hasOBONamespace>
        <oboInOwl:id>GAZ:00250872</oboInOwl:id>
        <rdfs:label>Choghakor Marsh</rdfs:label>
    </owl:NamedIndividual>
    


    <!-- http://purl.obolibrary.org/obo/GAZ_00250873 -->

    <owl:NamedIndividual rdf:about="http://purl.obolibrary.org/obo/GAZ_00250873">
        <obo:RO_0001025 rdf:resource="http://purl.obolibrary.org/obo/GAZ_00004481"/>
        <obo:IAO_0000115>A wetland. A freshwater marsh. Located in the upper drainage of the Karun River in the Zagros Mountains, about 25 km southwest of Borujen and 75 km west-southwest of Shahreza, Chaharmahal and Bakhtiari.</obo:IAO_0000115>
        <oboInOwl:hasOBONamespace>GAZ</oboInOwl:hasOBONamespace>
        <oboInOwl:id>GAZ:00250873</oboInOwl:id>
        <rdfs:label>Gandoman Marsh</rdfs:label>
    </owl:NamedIndividual>
    


    <!-- http://purl.obolibrary.org/obo/GAZ_00250877 -->

    <owl:NamedIndividual rdf:about="http://purl.obolibrary.org/obo/GAZ_00250877">
        <obo:RO_0001025 rdf:resource="http://purl.obolibrary.org/obo/GAZ_00004481"/>
        <obo:IAO_0000115>A group of freshwater lakes. Located in the rolling uplands of the high Zagros Mountains about 65 km WNW of Shiraz, Fars.</obo:IAO_0000115>
        <oboInOwl:hasOBONamespace>GAZ</oboInOwl:hasOBONamespace>
        <oboInOwl:id>GAZ:00250877</oboInOwl:id>
        <rdfs:label>Haft Barm</rdfs:label>
    </owl:NamedIndividual>
    


    <!-- http://purl.obolibrary.org/obo/GAZ_00250878 -->

    <owl:NamedIndividual rdf:about="http://purl.obolibrary.org/obo/GAZ_00250878">
        <obo:RO_0001025 rdf:resource="http://purl.obolibrary.org/obo/GAZ_00004481"/>
        <obo:IAO_0000115>A wetland. A largely seasonal freshwater lake and marsh at 2,000 m elevation in the Zagros Mountains. A Ramsar Site.</obo:IAO_0000115>
        <oboInOwl:hasOBONamespace>GAZ</oboInOwl:hasOBONamespace>
        <oboInOwl:id>GAZ:00250878</oboInOwl:id>
        <rdfs:label>Dasht-e Arjan</rdfs:label>
    </owl:NamedIndividual>
    


    <!-- http://purl.obolibrary.org/obo/GAZ_00250879 -->

    <owl:NamedIndividual rdf:about="http://purl.obolibrary.org/obo/GAZ_00250879">
        <obo:RO_0001025 rdf:resource="http://purl.obolibrary.org/obo/GAZ_00004481"/>
        <obo:IAO_0000115>A brackish/saline lake. At 853 m in the Zagros foothills. A Ramsar Site.</obo:IAO_0000115>
        <oboInOwl:hasOBONamespace>GAZ</oboInOwl:hasOBONamespace>
        <oboInOwl:id>GAZ:00250879</oboInOwl:id>
        <rdfs:label>Lake Parishan</rdfs:label>
    </owl:NamedIndividual>
    


    <!-- http://purl.obolibrary.org/obo/GAZ_00250880 -->

    <owl:NamedIndividual rdf:about="http://purl.obolibrary.org/obo/GAZ_00250880">
        <obo:RO_0001025 rdf:resource="http://purl.obolibrary.org/obo/GAZ_00004481"/>
        <obo:IAO_0000115>A saline lake. Located in an intermontane basin in the Zagros Mountains about 20 km SE of Shiraz, Fars.</obo:IAO_0000115>
        <oboInOwl:hasOBONamespace>GAZ</oboInOwl:hasOBONamespace>
        <oboInOwl:id>GAZ:00250880</oboInOwl:id>
        <rdfs:label>Lake Maharlu</rdfs:label>
    </owl:NamedIndividual>
    


    <!-- http://purl.obolibrary.org/obo/GAZ_00250881 -->

    <owl:NamedIndividual rdf:about="http://purl.obolibrary.org/obo/GAZ_00250881">
        <obo:RO_0001025 rdf:resource="http://purl.obolibrary.org/obo/GAZ_00250884"/>
        <obo:IAO_0000115>A saline lake. Located in a large intermontane basin in the eastern Zagros Mountains, 50-160 km east of Shiraz, Fars. A Ramsar Site.</obo:IAO_0000115>
        <oboInOwl:hasOBONamespace>GAZ</oboInOwl:hasOBONamespace>
        <oboInOwl:id>GAZ:00250881</oboInOwl:id>
        <rdfs:label>Lake Bakhtegan</rdfs:label>
    </owl:NamedIndividual>
    


    <!-- http://purl.obolibrary.org/obo/GAZ_00250882 -->

    <owl:NamedIndividual rdf:about="http://purl.obolibrary.org/obo/GAZ_00250882">
        <obo:RO_0001025 rdf:resource="http://purl.obolibrary.org/obo/GAZ_00250884"/>
        <obo:IAO_0000115>A saline lake. Located in a large intermontane basin in the eastern Zagros Mountains, 50-160 km east of Shiraz, Fars. A Ramsar Site.</obo:IAO_0000115>
        <oboInOwl:hasOBONamespace>GAZ</oboInOwl:hasOBONamespace>
        <oboInOwl:id>GAZ:00250882</oboInOwl:id>
        <rdfs:label>Lake Tashk</rdfs:label>
    </owl:NamedIndividual>
    


    <!-- http://purl.obolibrary.org/obo/GAZ_00250883 -->

    <owl:NamedIndividual rdf:about="http://purl.obolibrary.org/obo/GAZ_00250883">
        <obo:RO_0001025 rdf:resource="http://purl.obolibrary.org/obo/GAZ_00250885"/>
        <obo:IAO_0000115>A freshwater marsh. Located along the lower Kur River.</obo:IAO_0000115>
        <oboInOwl:hasOBONamespace>GAZ</oboInOwl:hasOBONamespace>
        <oboInOwl:id>GAZ:00250883</oboInOwl:id>
        <rdfs:label>Kamjan Marshes</rdfs:label>
    </owl:NamedIndividual>
    


    <!-- http://purl.obolibrary.org/obo/GAZ_00250884 -->

    <owl:NamedIndividual rdf:about="http://purl.obolibrary.org/obo/GAZ_00250884">
        <obo:RO_0001025 rdf:resource="http://purl.obolibrary.org/obo/GAZ_00250885"/>
        <obo:IAO_0000115>A protected area. Established (as Wildlife Refuge): 1970. A Ramsar Site.</obo:IAO_0000115>
        <oboInOwl:hasOBONamespace>GAZ</oboInOwl:hasOBONamespace>
        <oboInOwl:id>GAZ:00250884</oboInOwl:id>
        <rdfs:label>Bakhtegan Wildlife Refuge</rdfs:label>
    </owl:NamedIndividual>
    


    <!-- http://purl.obolibrary.org/obo/GAZ_00250885 -->

    <owl:NamedIndividual rdf:about="http://purl.obolibrary.org/obo/GAZ_00250885">
        <obo:RO_0001025 rdf:resource="http://purl.obolibrary.org/obo/GAZ_00004481"/>
        <obo:IAO_0000115>A drainage basin in the southeastern Zagros Mountains.</obo:IAO_0000115>
        <oboInOwl:hasOBONamespace>GAZ</oboInOwl:hasOBONamespace>
        <oboInOwl:id>GAZ:00250885</oboInOwl:id>
        <rdfs:label>Neiris Basin</rdfs:label>
    </owl:NamedIndividual>
    


    <!-- http://purl.obolibrary.org/obo/GAZ_00250886 -->

    <owl:NamedIndividual rdf:about="http://purl.obolibrary.org/obo/GAZ_00250886">
        <obo:RO_0001025 rdf:resource="http://purl.obolibrary.org/obo/GAZ_00004481"/>
        <obo:IAO_0000115>A lake. Located in an intermontane basin in the southern Zagros, about 35 km SSE of Jahrom, Fars.</obo:IAO_0000115>
        <oboInOwl:hasOBONamespace>GAZ</oboInOwl:hasOBONamespace>
        <oboInOwl:id>GAZ:00250886</oboInOwl:id>
        <rdfs:label>Harm Lake</rdfs:label>
    </owl:NamedIndividual>
    


    <!-- http://purl.obolibrary.org/obo/GAZ_00250909 -->

    <owl:NamedIndividual rdf:about="http://purl.obolibrary.org/obo/GAZ_00250909">
        <obo:RO_0001025 rdf:resource="http://purl.obolibrary.org/obo/GAZ_00005295"/>
        <obo:IAO_0000115>A small sandy island with fringing coral reefs in the northern Persian Gulf.</obo:IAO_0000115>
        <oboInOwl:hasOBONamespace>GAZ</oboInOwl:hasOBONamespace>
        <oboInOwl:id>GAZ:00250909</oboInOwl:id>
        <rdfs:label>Jazireh-ye Kharku</rdfs:label>
    </owl:NamedIndividual>
    


    <!-- http://purl.obolibrary.org/obo/GAZ_00250911 -->

    <owl:NamedIndividual rdf:about="http://purl.obolibrary.org/obo/GAZ_00250911">
        <obo:IAO_0000115>A river.</obo:IAO_0000115>
        <oboInOwl:hasOBONamespace>GAZ</oboInOwl:hasOBONamespace>
        <oboInOwl:id>GAZ:00250911</oboInOwl:id>
        <rdfs:label>Helleh Rud</rdfs:label>
    </owl:NamedIndividual>
    


    <!-- http://purl.obolibrary.org/obo/GAZ_00250912 -->

    <owl:NamedIndividual rdf:about="http://purl.obolibrary.org/obo/GAZ_00250912">
        <obo:RO_0001025 rdf:resource="http://purl.obolibrary.org/obo/GAZ_00250911"/>
        <obo:IAO_0000115>The delta of the Helleh River.</obo:IAO_0000115>
        <oboInOwl:hasOBONamespace>GAZ</oboInOwl:hasOBONamespace>
        <oboInOwl:id>GAZ:00250912</oboInOwl:id>
        <rdfs:label>Helleh Delta</rdfs:label>
    </owl:NamedIndividual>
    


    <!-- http://purl.obolibrary.org/obo/GAZ_00250913 -->

    <owl:NamedIndividual rdf:about="http://purl.obolibrary.org/obo/GAZ_00250913">
        <obo:RO_0001025 rdf:resource="http://purl.obolibrary.org/obo/GAZ_00005295"/>
        <obo:IAO_0000115>A shallow sea bay.</obo:IAO_0000115>
        <oboInOwl:hasOBONamespace>GAZ</oboInOwl:hasOBONamespace>
        <oboInOwl:id>GAZ:00250913</oboInOwl:id>
        <rdfs:label>Bushehr Bay</rdfs:label>
    </owl:NamedIndividual>
    


    <!-- http://purl.obolibrary.org/obo/GAZ_00250917 -->

    <owl:NamedIndividual rdf:about="http://purl.obolibrary.org/obo/GAZ_00250917">
        <obo:RO_0001025 rdf:resource="http://purl.obolibrary.org/obo/GAZ_00005295"/>
        <obo:IAO_0000115>A sandy inshore island. Located in the Persian Gulf about 40 km southeast of the Monde River Delta.</obo:IAO_0000115>
        <oboInOwl:hasOBONamespace>GAZ</oboInOwl:hasOBONamespace>
        <oboInOwl:id>GAZ:00250917</oboInOwl:id>
        <rdfs:label>Nakhilu Island</rdfs:label>
    </owl:NamedIndividual>
    


    <!-- http://purl.obolibrary.org/obo/GAZ_00250918 -->

    <owl:NamedIndividual rdf:about="http://purl.obolibrary.org/obo/GAZ_00250918">
        <obo:RO_0001025 rdf:resource="http://purl.obolibrary.org/obo/GAZ_00005295"/>
        <obo:IAO_0000115>A sandy inshore island. Located in the Persian Gulf about 40 km southeast of the Monde River Delta.</obo:IAO_0000115>
        <oboInOwl:hasOBONamespace>GAZ</oboInOwl:hasOBONamespace>
        <oboInOwl:id>GAZ:00250918</oboInOwl:id>
        <rdfs:label>Morghu Island</rdfs:label>
    </owl:NamedIndividual>
    


    <!-- http://purl.obolibrary.org/obo/GAZ_00250919 -->

    <owl:NamedIndividual rdf:about="http://purl.obolibrary.org/obo/GAZ_00250919">
        <obo:RO_0001025 rdf:resource="http://purl.obolibrary.org/obo/GAZ_00005295"/>
        <obo:IAO_0000115>A sandy inshore island. Located in the Persian Gulf about 40 km southeast of the Monde River Delta.</obo:IAO_0000115>
        <oboInOwl:hasOBONamespace>GAZ</oboInOwl:hasOBONamespace>
        <oboInOwl:id>GAZ:00250919</oboInOwl:id>
        <rdfs:label>Umm al Korm Island</rdfs:label>
    </owl:NamedIndividual>
    


    <!-- http://purl.obolibrary.org/obo/GAZ_00250920 -->

    <owl:NamedIndividual rdf:about="http://purl.obolibrary.org/obo/GAZ_00250920">
        <obo:RO_0001025 rdf:resource="http://purl.obolibrary.org/obo/GAZ_00005295"/>
        <obo:IAO_0000115>Two small rocky offshore islands in the south-central Persian Gulf, 45 km southwest of Bandar Lengeh.</obo:IAO_0000115>
        <oboInOwl:hasOBONamespace>GAZ</oboInOwl:hasOBONamespace>
        <oboInOwl:id>GAZ:00250920</oboInOwl:id>
        <rdfs:label>Faror Islands</rdfs:label>
    </owl:NamedIndividual>
    


    <!-- http://purl.obolibrary.org/obo/GAZ_00250921 -->

    <owl:NamedIndividual rdf:about="http://purl.obolibrary.org/obo/GAZ_00250921">
        <obo:RO_0001025 rdf:resource="http://purl.obolibrary.org/obo/GAZ_00250920"/>
        <obo:IAO_0000115>A protected area.</obo:IAO_0000115>
        <oboInOwl:hasOBONamespace>GAZ</oboInOwl:hasOBONamespace>
        <oboInOwl:id>GAZ:00250921</oboInOwl:id>
        <rdfs:label>Faror Protected Area</rdfs:label>
    </owl:NamedIndividual>
    


    <!-- http://purl.obolibrary.org/obo/GAZ_00250922 -->

    <owl:NamedIndividual rdf:about="http://purl.obolibrary.org/obo/GAZ_00250922">
        <obo:RO_0001025 rdf:resource="http://purl.obolibrary.org/obo/GAZ_00005295"/>
        <obo:IAO_0000115>A narrow strait separating the Iranian island of Qeshm from the Iranian mainland.</obo:IAO_0000115>
        <oboInOwl:hasOBONamespace>GAZ</oboInOwl:hasOBONamespace>
        <oboInOwl:id>GAZ:00250922</oboInOwl:id>
        <rdfs:label>Khouran Strait</rdfs:label>
    </owl:NamedIndividual>
    


    <!-- http://purl.obolibrary.org/obo/GAZ_00250926 -->

    <owl:NamedIndividual rdf:about="http://purl.obolibrary.org/obo/GAZ_00250926">
        <obo:IAO_0000115>A shallow bay.</obo:IAO_0000115>
        <oboInOwl:hasOBONamespace>GAZ</oboInOwl:hasOBONamespace>
        <oboInOwl:id>GAZ:00250926</oboInOwl:id>
        <rdfs:label>Khor Tiab</rdfs:label>
    </owl:NamedIndividual>
    


    <!-- http://purl.obolibrary.org/obo/GAZ_00250927 -->

    <owl:NamedIndividual rdf:about="http://purl.obolibrary.org/obo/GAZ_00250927">
        <obo:IAO_0000115>A shallow bay.</obo:IAO_0000115>
        <oboInOwl:hasOBONamespace>GAZ</oboInOwl:hasOBONamespace>
        <oboInOwl:id>GAZ:00250927</oboInOwl:id>
        <rdfs:label>Khor Kolahy</rdfs:label>
    </owl:NamedIndividual>
    


    <!-- http://purl.obolibrary.org/obo/GAZ_00250950 -->

    <owl:NamedIndividual rdf:about="http://purl.obolibrary.org/obo/GAZ_00250950">
        <obo:RO_0001025 rdf:resource="http://purl.obolibrary.org/obo/GAZ_00057476"/>
        <obo:RO_0001025 rdf:resource="http://purl.obolibrary.org/obo/GAZ_02000615"/>
        <obo:IAO_0000115>A multi-purpose arch dam located on the Lesser Zab River approximately 220 km upstream from its confluence with the Tigris River. The site is located adjacent to the town of Dukan in the north of As Sulaymaniyah Governorate, Iraq. Constructed 1954-1959.</obo:IAO_0000115>
        <oboInOwl:hasOBONamespace>GAZ</oboInOwl:hasOBONamespace>
        <oboInOwl:id>GAZ:00250950</oboInOwl:id>
        <rdfs:label>Dukan Dam</rdfs:label>
    </owl:NamedIndividual>
    


    <!-- http://purl.obolibrary.org/obo/GAZ_00250961 -->

    <owl:NamedIndividual rdf:about="http://purl.obolibrary.org/obo/GAZ_00250961">
        <obo:RO_0001025 rdf:resource="http://purl.obolibrary.org/obo/GAZ_02000620"/>
        <obo:IAO_0000115>Adiversion dam on the Diyala River 90km northeast of Baghdad, Iraq. The main purpose of the dam is to divert outflow of the Hemrin Dam (11km upstream) on the Diyala River to the Khalis and Sadr Al-Mushtarak canals for irrigation.</obo:IAO_0000115>
        <oboInOwl:hasOBONamespace>GAZ</oboInOwl:hasOBONamespace>
        <oboInOwl:id>GAZ:00250961</oboInOwl:id>
        <rdfs:label>Diyala Weir</rdfs:label>
    </owl:NamedIndividual>
    


    <!-- http://purl.obolibrary.org/obo/GAZ_00250962 -->

    <owl:NamedIndividual rdf:about="http://purl.obolibrary.org/obo/GAZ_00250962">
        <obo:RO_0001025 rdf:resource="http://purl.obolibrary.org/obo/GAZ_02000620"/>
        <obo:IAO_0000115>A dam on the Diyala River 100 km northeast of Baghdad, Iraq. The main purpose of the dam is to control flood waters on the Diyala River along with storing water for irrigation and to support a 50 MW hydroelectricity station. Impounds Lake Hamrin. Constructed 1981.</obo:IAO_0000115>
        <oboInOwl:hasOBONamespace>GAZ</oboInOwl:hasOBONamespace>
        <oboInOwl:id>GAZ:00250962</oboInOwl:id>
        <rdfs:label>Hemrin Dam</rdfs:label>
    </owl:NamedIndividual>
    


    <!-- http://purl.obolibrary.org/obo/GAZ_00250963 -->

    <owl:NamedIndividual rdf:about="http://purl.obolibrary.org/obo/GAZ_00250963">
        <obo:RO_0001025 rdf:resource="http://purl.obolibrary.org/obo/GAZ_00250964"/>
        <obo:IAO_0000115>A District of Baghdad.</obo:IAO_0000115>
        <oboInOwl:hasOBONamespace>GAZ</oboInOwl:hasOBONamespace>
        <oboInOwl:id>GAZ:00250963</oboInOwl:id>
        <rdfs:label>Rusafa District</rdfs:label>
    </owl:NamedIndividual>
    


    <!-- http://purl.obolibrary.org/obo/GAZ_00250964 -->

    <owl:NamedIndividual rdf:about="http://purl.obolibrary.org/obo/GAZ_00250964">
        <obo:RO_0001025 rdf:resource="http://purl.obolibrary.org/obo/GAZ_00010360"/>
        <obo:IAO_0000115>The east-bank settlement of Baghdad, Iraq, or the eastern shore of the river Tigris.</obo:IAO_0000115>
        <oboInOwl:hasOBONamespace>GAZ</oboInOwl:hasOBONamespace>
        <oboInOwl:id>GAZ:00250964</oboInOwl:id>
        <rdfs:label>Rusafa</rdfs:label>
    </owl:NamedIndividual>
    


    <!-- http://purl.obolibrary.org/obo/GAZ_00250965 -->

    <owl:NamedIndividual rdf:about="http://purl.obolibrary.org/obo/GAZ_00250965">
        <obo:RO_0001025 rdf:resource="http://purl.obolibrary.org/obo/GAZ_00250964"/>
        <obo:IAO_0000115>A District of Baghdad.</obo:IAO_0000115>
        <oboInOwl:hasOBONamespace>GAZ</oboInOwl:hasOBONamespace>
        <oboInOwl:id>GAZ:00250965</oboInOwl:id>
        <rdfs:label>Thawra District</rdfs:label>
    </owl:NamedIndividual>
    


    <!-- http://purl.obolibrary.org/obo/GAZ_00250966 -->

    <owl:NamedIndividual rdf:about="http://purl.obolibrary.org/obo/GAZ_00250966">
        <obo:RO_0001025 rdf:resource="http://purl.obolibrary.org/obo/GAZ_00250964"/>
        <obo:IAO_0000115>A District of Baghdad.</obo:IAO_0000115>
        <oboInOwl:hasOBONamespace>GAZ</oboInOwl:hasOBONamespace>
        <oboInOwl:id>GAZ:00250966</oboInOwl:id>
        <rdfs:label>Karadah District</rdfs:label>
    </owl:NamedIndividual>
    


    <!-- http://purl.obolibrary.org/obo/GAZ_00250967 -->

    <owl:NamedIndividual rdf:about="http://purl.obolibrary.org/obo/GAZ_00250967">
        <obo:RO_0001025 rdf:resource="http://purl.obolibrary.org/obo/GAZ_00250964"/>
        <obo:IAO_0000115>A District of Baghdad.</obo:IAO_0000115>
        <oboInOwl:hasOBONamespace>GAZ</oboInOwl:hasOBONamespace>
        <oboInOwl:id>GAZ:00250967</oboInOwl:id>
        <rdfs:label>7 Nissan District</rdfs:label>
    </owl:NamedIndividual>
    


    <!-- http://purl.obolibrary.org/obo/GAZ_00250968 -->

    <owl:NamedIndividual rdf:about="http://purl.obolibrary.org/obo/GAZ_00250968">
        <obo:RO_0001025 rdf:resource="http://purl.obolibrary.org/obo/GAZ_00010360"/>
        <obo:IAO_0000115>The western half of Baghdad, Iraq.</obo:IAO_0000115>
        <oboInOwl:hasOBONamespace>GAZ</oboInOwl:hasOBONamespace>
        <oboInOwl:id>GAZ:00250968</oboInOwl:id>
        <rdfs:label>Karkh</rdfs:label>
    </owl:NamedIndividual>
    


    <!-- http://purl.obolibrary.org/obo/GAZ_00250969 -->

    <owl:NamedIndividual rdf:about="http://purl.obolibrary.org/obo/GAZ_00250969">
        <obo:RO_0001025 rdf:resource="http://purl.obolibrary.org/obo/GAZ_00250968"/>
        <obo:IAO_0000115>A District of Baghdad.</obo:IAO_0000115>
        <oboInOwl:hasOBONamespace>GAZ</oboInOwl:hasOBONamespace>
        <oboInOwl:id>GAZ:00250969</oboInOwl:id>
        <rdfs:label>Karkh District</rdfs:label>
    </owl:NamedIndividual>
    


    <!-- http://purl.obolibrary.org/obo/GAZ_00250970 -->

    <owl:NamedIndividual rdf:about="http://purl.obolibrary.org/obo/GAZ_00250970">
        <obo:RO_0001025 rdf:resource="http://purl.obolibrary.org/obo/GAZ_00250968"/>
        <obo:IAO_0000115>A District of Baghdad.</obo:IAO_0000115>
        <oboInOwl:hasOBONamespace>GAZ</oboInOwl:hasOBONamespace>
        <oboInOwl:id>GAZ:00250970</oboInOwl:id>
        <rdfs:label>Kadhimiya District</rdfs:label>
    </owl:NamedIndividual>
    


    <!-- http://purl.obolibrary.org/obo/GAZ_00250971 -->

    <owl:NamedIndividual rdf:about="http://purl.obolibrary.org/obo/GAZ_00250971">
        <obo:RO_0001025 rdf:resource="http://purl.obolibrary.org/obo/GAZ_00250968"/>
        <obo:IAO_0000115>A District of Baghdad.</obo:IAO_0000115>
        <oboInOwl:hasOBONamespace>GAZ</oboInOwl:hasOBONamespace>
        <oboInOwl:id>GAZ:00250971</oboInOwl:id>
        <rdfs:label>Mansour District</rdfs:label>
    </owl:NamedIndividual>
    


    <!-- http://purl.obolibrary.org/obo/GAZ_00250972 -->

    <owl:NamedIndividual rdf:about="http://purl.obolibrary.org/obo/GAZ_00250972">
        <obo:RO_0001025 rdf:resource="http://purl.obolibrary.org/obo/GAZ_00250968"/>
        <obo:IAO_0000115>A District of Baghdad.</obo:IAO_0000115>
        <oboInOwl:hasOBONamespace>GAZ</oboInOwl:hasOBONamespace>
        <oboInOwl:id>GAZ:00250972</oboInOwl:id>
        <rdfs:label>Rasheed District</rdfs:label>
    </owl:NamedIndividual>
    


    <!-- http://purl.obolibrary.org/obo/GAZ_00250982 -->

    <owl:NamedIndividual rdf:about="http://purl.obolibrary.org/obo/GAZ_00250982">
        <obo:RO_0001025 rdf:resource="http://purl.obolibrary.org/obo/GAZ_02000621"/>
        <obo:IAO_0000115>A wetland. Located in the valley of the Little Zab River, about 50 km WSW of Kirkuk.</obo:IAO_0000115>
        <oboInOwl:hasOBONamespace>GAZ</oboInOwl:hasOBONamespace>
        <oboInOwl:id>GAZ:00250982</oboInOwl:id>
        <rdfs:label>Haweija Marshes</rdfs:label>
    </owl:NamedIndividual>
    


    <!-- http://purl.obolibrary.org/obo/GAZ_00250983 -->

    <owl:NamedIndividual rdf:about="http://purl.obolibrary.org/obo/GAZ_00250983">
        <obo:RO_0001025 rdf:resource="http://purl.obolibrary.org/obo/GAZ_00030453"/>
        <obo:IAO_0000115>An earth-fill dam on the Euphrates, north of Haditha (Iraq), creating Lake Qadisiyah (Buhayrat al-Qadisiyyah). Constructed 1977-1987.</obo:IAO_0000115>
        <oboInOwl:hasOBONamespace>GAZ</oboInOwl:hasOBONamespace>
        <oboInOwl:id>GAZ:00250983</oboInOwl:id>
        <rdfs:label>Haditha Dam</rdfs:label>
    </owl:NamedIndividual>
    


    <!-- http://purl.obolibrary.org/obo/GAZ_00250984 -->

    <owl:NamedIndividual rdf:about="http://purl.obolibrary.org/obo/GAZ_00250984">
        <obo:IAO_0000115>A man-made reservoir in Al-Anbar, Iraq. Impounded by Haditha Dam.</obo:IAO_0000115>
        <oboInOwl:hasOBONamespace>GAZ</oboInOwl:hasOBONamespace>
        <oboInOwl:id>GAZ:00250984</oboInOwl:id>
        <rdfs:label>Lake Qadisiyah</rdfs:label>
    </owl:NamedIndividual>
    


    <!-- http://purl.obolibrary.org/obo/GAZ_00250985 -->

    <owl:NamedIndividual rdf:about="http://purl.obolibrary.org/obo/GAZ_00250985">
        <obo:RO_0001025 rdf:resource="http://purl.obolibrary.org/obo/GAZ_02000622"/>
        <obo:IAO_0000115>A populated place. A city in central Iraq.</obo:IAO_0000115>
        <oboInOwl:hasOBONamespace>GAZ</oboInOwl:hasOBONamespace>
        <oboInOwl:id>GAZ:00250985</oboInOwl:id>
        <rdfs:label>Iskandariya</rdfs:label>
    </owl:NamedIndividual>
    


    <!-- http://purl.obolibrary.org/obo/GAZ_00250986 -->

    <owl:NamedIndividual rdf:about="http://purl.obolibrary.org/obo/GAZ_00250986">
        <obo:RO_0001025 rdf:resource="http://purl.obolibrary.org/obo/GAZ_02000622"/>
        <obo:IAO_0000115>A populated place. A city on the Euphrates River in Iraq.</obo:IAO_0000115>
        <oboInOwl:hasOBONamespace>GAZ</oboInOwl:hasOBONamespace>
        <oboInOwl:id>GAZ:00250986</oboInOwl:id>
        <rdfs:label>Saddat al Hindiyah</rdfs:label>
    </owl:NamedIndividual>
    


    <!-- http://purl.obolibrary.org/obo/GAZ_00250988 -->

    <owl:NamedIndividual rdf:about="http://purl.obolibrary.org/obo/GAZ_00250988">
        <obo:RO_0001025 rdf:resource="http://purl.obolibrary.org/obo/GAZ_00193963"/>
        <obo:IAO_0000115>A lake.</obo:IAO_0000115>
        <oboInOwl:hasOBONamespace>GAZ</oboInOwl:hasOBONamespace>
        <oboInOwl:id>GAZ:00250988</oboInOwl:id>
        <rdfs:label>Haur az-Zikri</rdfs:label>
    </owl:NamedIndividual>
    


    <!-- http://purl.obolibrary.org/obo/GAZ_00250990 -->

    <owl:NamedIndividual rdf:about="http://purl.obolibrary.org/obo/GAZ_00250990">
        <obo:RO_0001025 rdf:resource="http://purl.obolibrary.org/obo/GAZ_00004492"/>
        <obo:IAO_0000115>A marshy region adjoining the Persian Gulf in the extreme south-east of Iraq, between and to the south-east of the cities of Basra (Iraq) and Abadan (Iran).</obo:IAO_0000115>
        <oboInOwl:hasOBONamespace>GAZ</oboInOwl:hasOBONamespace>
        <oboInOwl:id>GAZ:00250990</oboInOwl:id>
        <rdfs:label>Al-Faw Peninsula</rdfs:label>
    </owl:NamedIndividual>
    


    <!-- http://purl.obolibrary.org/obo/GAZ_00250991 -->

    <owl:NamedIndividual rdf:about="http://purl.obolibrary.org/obo/GAZ_00250991">
        <obo:RO_0001025 rdf:resource="http://purl.obolibrary.org/obo/GAZ_00057476"/>
        <obo:IAO_0000115>A ridge of mountains located in Iraqi Kurdistan (northwestern Iraq). It is situated near Sinjar.</obo:IAO_0000115>
        <oboInOwl:hasOBONamespace>GAZ</oboInOwl:hasOBONamespace>
        <oboInOwl:id>GAZ:00250991</oboInOwl:id>
        <rdfs:label>Sinjar Mountains</rdfs:label>
    </owl:NamedIndividual>
    


    <!-- http://purl.obolibrary.org/obo/GAZ_00250992 -->

    <owl:NamedIndividual rdf:about="http://purl.obolibrary.org/obo/GAZ_00250992">
        <obo:RO_0001025 rdf:resource="http://purl.obolibrary.org/obo/GAZ_00030825"/>
        <obo:IAO_0000115>A populated place. A city in Iraq and capital of Kirkuk Governorate.</obo:IAO_0000115>
        <oboInOwl:hasOBONamespace>GAZ</oboInOwl:hasOBONamespace>
        <oboInOwl:id>GAZ:00250992</oboInOwl:id>
        <rdfs:label>Kirkuk</rdfs:label>
    </owl:NamedIndividual>
    


    <!-- http://purl.obolibrary.org/obo/GAZ_00250993 -->

    <owl:NamedIndividual rdf:about="http://purl.obolibrary.org/obo/GAZ_00250993">
        <obo:RO_0001025 rdf:resource="http://purl.obolibrary.org/obo/GAZ_00004481"/>
        <obo:RO_0001025 rdf:resource="http://purl.obolibrary.org/obo/GAZ_00057476"/>
        <obo:IAO_0000115>A paleontological site. A cave located in the Zagros Mountains of Kurdistan in Iraq.</obo:IAO_0000115>
        <oboInOwl:hasOBONamespace>GAZ</oboInOwl:hasOBONamespace>
        <oboInOwl:id>GAZ:00250993</oboInOwl:id>
        <rdfs:label>Shanidar Cave</rdfs:label>
    </owl:NamedIndividual>
    


    <!-- http://purl.obolibrary.org/obo/GAZ_00250994 -->

    <owl:NamedIndividual rdf:about="http://purl.obolibrary.org/obo/GAZ_00250994">
        <obo:RO_0001025 rdf:resource="http://purl.obolibrary.org/obo/GAZ_00030835"/>
        <obo:IAO_0000115>A dam ocated on the Tigris River in the western governorate of Ninawa, upstream of the city of Mosul. Constructed 1980-1986.</obo:IAO_0000115>
        <oboInOwl:hasOBONamespace>GAZ</oboInOwl:hasOBONamespace>
        <oboInOwl:id>GAZ:00250994</oboInOwl:id>
        <rdfs:label>Mosul Dam</rdfs:label>
    </owl:NamedIndividual>
    


    <!-- http://purl.obolibrary.org/obo/GAZ_00250995 -->

    <owl:NamedIndividual rdf:about="http://purl.obolibrary.org/obo/GAZ_00250995">
        <obo:IAO_0000115>An unfinished multi-purpose rock-fill dam on the Greater Zab River 60 km northeast of Arbil, Iraq. Constructed 1979-.</obo:IAO_0000115>
        <oboInOwl:hasOBONamespace>GAZ</oboInOwl:hasOBONamespace>
        <oboInOwl:id>GAZ:00250995</oboInOwl:id>
        <rdfs:label>Bokhme Dam</rdfs:label>
    </owl:NamedIndividual>
    


    <!-- http://purl.obolibrary.org/obo/GAZ_00250996 -->

    <owl:NamedIndividual rdf:about="http://purl.obolibrary.org/obo/GAZ_00250996">
        <obo:IAO_0000115>A man-made lake approximately 50 km north-east of the Baquba, in Iraq&apos;s Diyala province. Impounded by Hemrin Dam. Constructed 1981.</obo:IAO_0000115>
        <oboInOwl:hasOBONamespace>GAZ</oboInOwl:hasOBONamespace>
        <oboInOwl:id>GAZ:00250996</oboInOwl:id>
        <rdfs:label>Lake Hemrin</rdfs:label>
    </owl:NamedIndividual>
    


    <!-- http://purl.obolibrary.org/obo/GAZ_00250997 -->

    <owl:NamedIndividual rdf:about="http://purl.obolibrary.org/obo/GAZ_00250997">
        <obo:RO_0001025 rdf:resource="http://purl.obolibrary.org/obo/GAZ_02000615"/>
        <obo:IAO_0000115>A mutli-purpose high-zoned embankment dam located on the Sirwan River in northern As Sulaymaniyah Governorate, Kurdistan. Constructed 1956-1961.</obo:IAO_0000115>
        <oboInOwl:hasOBONamespace>GAZ</oboInOwl:hasOBONamespace>
        <oboInOwl:id>GAZ:00250997</oboInOwl:id>
        <rdfs:label>Darbandikhan Dam</rdfs:label>
    </owl:NamedIndividual>
    


    <!-- http://purl.obolibrary.org/obo/GAZ_00250998 -->

    <owl:NamedIndividual rdf:about="http://purl.obolibrary.org/obo/GAZ_00250998">
        <rdf:type rdf:resource="http://purl.obolibrary.org/obo/ENVO_00000074"/>
        <obo:RO_0001025 rdf:resource="http://purl.obolibrary.org/obo/GAZ_00030447"/>
        <obo:IAO_0000115>A barrage on the Euphrates near Fallujah in Al Anbar Governorate, Iraq. Completed 1985.</obo:IAO_0000115>
        <oboInOwl:hasOBONamespace>GAZ</oboInOwl:hasOBONamespace>
        <oboInOwl:id>GAZ:00250998</oboInOwl:id>
        <rdfs:label>Fallujah Barrage</rdfs:label>
    </owl:NamedIndividual>
    


    <!-- http://purl.obolibrary.org/obo/GAZ_00250999 -->

    <owl:NamedIndividual rdf:about="http://purl.obolibrary.org/obo/GAZ_00250999">
        <obo:RO_0001025 rdf:resource="http://purl.obolibrary.org/obo/GAZ_02000627"/>
        <obo:IAO_0000115>A diversion dam on the Euphrates River adjacent (east) of Ramadi, Iraq. The main purpose of the dam is to divert floodwater in the Euphrates River to Lake Habbaniyah through a canal for storage.</obo:IAO_0000115>
        <oboInOwl:hasOBONamespace>GAZ</oboInOwl:hasOBONamespace>
        <oboInOwl:id>GAZ:00250999</oboInOwl:id>
        <rdfs:label>Ramadi Barrage</rdfs:label>
    </owl:NamedIndividual>
    


    <!-- http://purl.obolibrary.org/obo/GAZ_00251000 -->

    <owl:NamedIndividual rdf:about="http://purl.obolibrary.org/obo/GAZ_00251000">
        <obo:RO_0001025 rdf:resource="http://purl.obolibrary.org/obo/GAZ_00030486"/>
        <obo:IAO_0000115>A multi-purpose dam on the Tigris River adjacent (west) of Samarra and north of Baghdad, Iraq. The main purpose of the dam is to divert floodwater in the Tigris River to Lake Tharthar through the Thar Thar depression along with irrigation and a 75 MW hydroelectricity station. Impounds Samarra Lake.</obo:IAO_0000115>
        <oboInOwl:hasOBONamespace>GAZ</oboInOwl:hasOBONamespace>
        <oboInOwl:id>GAZ:00251000</oboInOwl:id>
        <rdfs:label>Samarra Dam</rdfs:label>
    </owl:NamedIndividual>
    


    <!-- http://purl.obolibrary.org/obo/GAZ_00251001 -->

    <owl:NamedIndividual rdf:about="http://purl.obolibrary.org/obo/GAZ_00251001">
        <obo:RO_0001025 rdf:resource="http://purl.obolibrary.org/obo/GAZ_02000616"/>
        <obo:IAO_0000115>A river.</obo:IAO_0000115>
        <oboInOwl:hasOBONamespace>GAZ</oboInOwl:hasOBONamespace>
        <oboInOwl:id>GAZ:00251001</oboInOwl:id>
        <rdfs:label>Al Uzaym River</rdfs:label>
    </owl:NamedIndividual>
    


    <!-- http://purl.obolibrary.org/obo/GAZ_00251002 -->

    <owl:NamedIndividual rdf:about="http://purl.obolibrary.org/obo/GAZ_00251002">
        <obo:RO_0001025 rdf:resource="http://purl.obolibrary.org/obo/GAZ_00251001"/>
        <obo:IAO_0000115>A multi-purpose embankment dam on the Al Uzaym River 133km northeast of Baghdad, Iraq.</obo:IAO_0000115>
        <oboInOwl:hasOBONamespace>GAZ</oboInOwl:hasOBONamespace>
        <oboInOwl:id>GAZ:00251002</oboInOwl:id>
        <rdfs:label>Adhaim Dam</rdfs:label>
    </owl:NamedIndividual>
    


    <!-- http://purl.obolibrary.org/obo/GAZ_00251003 -->

    <owl:NamedIndividual rdf:about="http://purl.obolibrary.org/obo/GAZ_00251003">
        <obo:IAO_0000115>A dam. Located on the Tigris River approximately 120 km downstream of Baghdad, in the town of Al Kut.</obo:IAO_0000115>
        <oboInOwl:hasOBONamespace>GAZ</oboInOwl:hasOBONamespace>
        <oboInOwl:id>GAZ:00251003</oboInOwl:id>
        <rdfs:label>Kut Barrage</rdfs:label>
    </owl:NamedIndividual>
    


    <!-- http://purl.obolibrary.org/obo/GAZ_00251004 -->

    <owl:NamedIndividual rdf:about="http://purl.obolibrary.org/obo/GAZ_00251004">
        <obo:RO_0001025 rdf:resource="http://purl.obolibrary.org/obo/GAZ_02000625"/>
        <obo:IAO_0000115>A river.</obo:IAO_0000115>
        <oboInOwl:hasOBONamespace>GAZ</oboInOwl:hasOBONamespace>
        <oboInOwl:id>GAZ:00251004</oboInOwl:id>
        <rdfs:label>Duhok River</rdfs:label>
    </owl:NamedIndividual>
    


    <!-- http://purl.obolibrary.org/obo/GAZ_00251005 -->

    <owl:NamedIndividual rdf:about="http://purl.obolibrary.org/obo/GAZ_00251005">
        <obo:RO_0001025 rdf:resource="http://purl.obolibrary.org/obo/GAZ_00251004"/>
        <obo:IAO_0000115>A dam.</obo:IAO_0000115>
        <oboInOwl:hasOBONamespace>GAZ</oboInOwl:hasOBONamespace>
        <oboInOwl:id>GAZ:00251005</oboInOwl:id>
        <rdfs:label>Duhok Dam</rdfs:label>
    </owl:NamedIndividual>
    


    <!-- http://purl.obolibrary.org/obo/GAZ_00251006 -->

    <owl:NamedIndividual rdf:about="http://purl.obolibrary.org/obo/GAZ_00251006">
        <obo:RO_0001025 rdf:resource="http://purl.obolibrary.org/obo/GAZ_02000621"/>
        <obo:IAO_0000115>A gravel-alluvial fill embankment dam located on Lesser Zab River approximately 130 km upstream from its confluence with the Tigris River. The dam is located directly north of the town of Dibis in Kirkuk Governorate, Iraq. The main-purpose of the Dibis Dam is to divert water from the Lesser Zab River into the Kirkuk Irrigation Project. Constructed 1960-1965.</obo:IAO_0000115>
        <oboInOwl:hasOBONamespace>GAZ</oboInOwl:hasOBONamespace>
        <oboInOwl:id>GAZ:00251006</oboInOwl:id>
        <rdfs:label>Dibis Dam</rdfs:label>
    </owl:NamedIndividual>
    


    <!-- http://purl.obolibrary.org/obo/GAZ_00251007 -->

    <owl:NamedIndividual rdf:about="http://purl.obolibrary.org/obo/GAZ_00251007">
        <obo:RO_0001025 rdf:resource="http://purl.obolibrary.org/obo/GAZ_00030835"/>
        <obo:IAO_0000115>An unfinished multi-purpose dam on the Tigris River 16 km northwest of Mosul, Iraq. Constructed 1990s-.</obo:IAO_0000115>
        <oboInOwl:hasOBONamespace>GAZ</oboInOwl:hasOBONamespace>
        <oboInOwl:id>GAZ:00251007</oboInOwl:id>
        <rdfs:label>Badush Dam</rdfs:label>
    </owl:NamedIndividual>
    


    <!-- http://purl.obolibrary.org/obo/GAZ_00251010 -->

    <owl:NamedIndividual rdf:about="http://purl.obolibrary.org/obo/GAZ_00251010">
        <obo:RO_0001025 rdf:resource="http://purl.obolibrary.org/obo/GAZ_00030486"/>
        <obo:IAO_0000115>A water storage reservoir. Impounded by Samarra Dam.</obo:IAO_0000115>
        <oboInOwl:hasOBONamespace>GAZ</oboInOwl:hasOBONamespace>
        <oboInOwl:id>GAZ:00251010</oboInOwl:id>
        <rdfs:label>Samarra Lake</rdfs:label>
    </owl:NamedIndividual>
    


    <!-- http://purl.obolibrary.org/obo/GAZ_00251012 -->

    <owl:NamedIndividual rdf:about="http://purl.obolibrary.org/obo/GAZ_00251012">
        <obo:RO_0001025 rdf:resource="http://purl.obolibrary.org/obo/GAZ_02000620"/>
        <obo:IAO_0000115>Wetlands. Located in the Diyala Valley about 10-20 km north-northeast of Baquba and 70 km north-northeast of Baghdad, Diyala Governorate.</obo:IAO_0000115>
        <oboInOwl:hasOBONamespace>GAZ</oboInOwl:hasOBONamespace>
        <oboInOwl:id>GAZ:00251012</oboInOwl:id>
        <rdfs:label>Baquba Wetlands</rdfs:label>
    </owl:NamedIndividual>
    


    <!-- http://purl.obolibrary.org/obo/GAZ_00251013 -->

    <owl:NamedIndividual rdf:about="http://purl.obolibrary.org/obo/GAZ_00251013">
        <obo:RO_0001025 rdf:resource="http://purl.obolibrary.org/obo/GAZ_00251012"/>
        <obo:IAO_0000115>A wetland. Much reduced in size by drainage in the 1970s.</obo:IAO_0000115>
        <oboInOwl:hasOBONamespace>GAZ</oboInOwl:hasOBONamespace>
        <oboInOwl:id>GAZ:00251013</oboInOwl:id>
        <rdfs:label>Haur Shaikh Sayed</rdfs:label>
    </owl:NamedIndividual>
    


    <!-- http://purl.obolibrary.org/obo/GAZ_00251014 -->

    <owl:NamedIndividual rdf:about="http://purl.obolibrary.org/obo/GAZ_00251014">
        <obo:RO_0001025 rdf:resource="http://purl.obolibrary.org/obo/GAZ_00251012"/>
        <obo:IAO_0000115>A wetland.</obo:IAO_0000115>
        <oboInOwl:hasOBONamespace>GAZ</oboInOwl:hasOBONamespace>
        <oboInOwl:id>GAZ:00251014</oboInOwl:id>
        <rdfs:label>Haur Abu Abbas</rdfs:label>
    </owl:NamedIndividual>
    


    <!-- http://purl.obolibrary.org/obo/GAZ_00251015 -->

    <owl:NamedIndividual rdf:about="http://purl.obolibrary.org/obo/GAZ_00251015">
        <obo:RO_0001025 rdf:resource="http://purl.obolibrary.org/obo/GAZ_00251012"/>
        <obo:IAO_0000115>A former freshwater lake. Drained in 1970s.</obo:IAO_0000115>
        <oboInOwl:hasOBONamespace>GAZ</oboInOwl:hasOBONamespace>
        <oboInOwl:id>GAZ:00251015</oboInOwl:id>
        <rdfs:label>Abdul Wand Lake</rdfs:label>
    </owl:NamedIndividual>
    


    <!-- http://purl.obolibrary.org/obo/GAZ_00251016 -->

    <owl:NamedIndividual rdf:about="http://purl.obolibrary.org/obo/GAZ_00251016">
        <obo:RO_0001025 rdf:resource="http://purl.obolibrary.org/obo/GAZ_00251012"/>
        <obo:IAO_0000115>A former freshwater lake. Drained in 1970s.</obo:IAO_0000115>
        <oboInOwl:hasOBONamespace>GAZ</oboInOwl:hasOBONamespace>
        <oboInOwl:id>GAZ:00251016</oboInOwl:id>
        <rdfs:label>Al Abara Lake</rdfs:label>
    </owl:NamedIndividual>
    


    <!-- http://purl.obolibrary.org/obo/GAZ_00251017 -->

    <owl:NamedIndividual rdf:about="http://purl.obolibrary.org/obo/GAZ_00251017">
        <obo:RO_0001025 rdf:resource="http://purl.obolibrary.org/obo/GAZ_00251012"/>
        <obo:IAO_0000115>A former freshwater lake. Drained in 1970s.</obo:IAO_0000115>
        <oboInOwl:hasOBONamespace>GAZ</oboInOwl:hasOBONamespace>
        <oboInOwl:id>GAZ:00251017</oboInOwl:id>
        <rdfs:label>Al Ahmar Lake</rdfs:label>
    </owl:NamedIndividual>
    


    <!-- http://purl.obolibrary.org/obo/GAZ_00251018 -->

    <owl:NamedIndividual rdf:about="http://purl.obolibrary.org/obo/GAZ_00251018">
        <obo:RO_0001025 rdf:resource="http://purl.obolibrary.org/obo/GAZ_00251012"/>
        <obo:IAO_0000115>A former freshwater lake. Drained in 1970s.</obo:IAO_0000115>
        <oboInOwl:hasOBONamespace>GAZ</oboInOwl:hasOBONamespace>
        <oboInOwl:id>GAZ:00251018</oboInOwl:id>
        <rdfs:label>Al Ugur Lake</rdfs:label>
    </owl:NamedIndividual>
    


    <!-- http://purl.obolibrary.org/obo/GAZ_00251019 -->

    <owl:NamedIndividual rdf:about="http://purl.obolibrary.org/obo/GAZ_00251019">
        <obo:RO_0001025 rdf:resource="http://purl.obolibrary.org/obo/GAZ_00010359"/>
        <obo:IAO_0000115>A wetland. A complex of shallow seasonal lagoons with a deeper, permanent central pool and a large area of seasonally flooded arable land in semi-desert country on the vast plains to the east of the Tigris River.</obo:IAO_0000115>
        <oboInOwl:hasOBONamespace>GAZ</oboInOwl:hasOBONamespace>
        <oboInOwl:id>GAZ:00251019</oboInOwl:id>
        <rdfs:label>Attariya Plains</rdfs:label>
    </owl:NamedIndividual>
    


    <!-- http://purl.obolibrary.org/obo/GAZ_00251023 -->

    <owl:NamedIndividual rdf:about="http://purl.obolibrary.org/obo/GAZ_00251023">
        <obo:RO_0001025 rdf:resource="http://purl.obolibrary.org/obo/GAZ_02000626"/>
        <obo:IAO_0000115>A former saline lake. Its area is now occupied by Lake Milh.</obo:IAO_0000115>
        <oboInOwl:hasOBONamespace>GAZ</oboInOwl:hasOBONamespace>
        <oboInOwl:id>GAZ:00251023</oboInOwl:id>
        <rdfs:label>Haur Abu Dibis</rdfs:label>
    </owl:NamedIndividual>
    


    <!-- http://purl.obolibrary.org/obo/GAZ_00251024 -->

    <owl:NamedIndividual rdf:about="http://purl.obolibrary.org/obo/GAZ_00251024">
        <obo:RO_0001025 rdf:resource="http://purl.obolibrary.org/obo/GAZ_02000626"/>
        <obo:IAO_0000115>A freshwater lake. Located a few km from the southeast corner of Lake Milh.</obo:IAO_0000115>
        <oboInOwl:hasOBONamespace>GAZ</oboInOwl:hasOBONamespace>
        <oboInOwl:id>GAZ:00251024</oboInOwl:id>
        <rdfs:label>Lake Usathe</rdfs:label>
    </owl:NamedIndividual>
    


    <!-- http://purl.obolibrary.org/obo/GAZ_00251025 -->

    <owl:NamedIndividual rdf:about="http://purl.obolibrary.org/obo/GAZ_00251025">
        <obo:RO_0001025 rdf:resource="http://purl.obolibrary.org/obo/GAZ_02000622"/>
        <obo:IAO_0000115>Wetlands. Located either side of the main Baghdad to Karbala road between the towns of Al Musayyib and Haswa, about 50 km south of Baghdad, Babil Governorate.</obo:IAO_0000115>
        <oboInOwl:hasOBONamespace>GAZ</oboInOwl:hasOBONamespace>
        <oboInOwl:id>GAZ:00251025</oboInOwl:id>
        <rdfs:label>Al Musayyib Wetlands</rdfs:label>
    </owl:NamedIndividual>
    


    <!-- http://purl.obolibrary.org/obo/GAZ_00251026 -->

    <owl:NamedIndividual rdf:about="http://purl.obolibrary.org/obo/GAZ_00251026">
        <obo:RO_0001025 rdf:resource="http://purl.obolibrary.org/obo/GAZ_02000622"/>
        <obo:IAO_0000115>A dam on the Euphrates River 5 km south of Al Musayyib and 65 km south of Baghdad, Babil Governorate.</obo:IAO_0000115>
        <oboInOwl:hasOBONamespace>GAZ</oboInOwl:hasOBONamespace>
        <oboInOwl:id>GAZ:00251026</oboInOwl:id>
        <rdfs:label>Al Hindiya Barrage</rdfs:label>
    </owl:NamedIndividual>
    


    <!-- http://purl.obolibrary.org/obo/GAZ_00251027 -->

    <owl:NamedIndividual rdf:about="http://purl.obolibrary.org/obo/GAZ_00251027">
        <obo:RO_0001025 rdf:resource="http://purl.obolibrary.org/obo/GAZ_02000622"/>
        <obo:IAO_0000115>A wetland. Located on the east bank of the Euphrates, about 35 km southsoutheast of Hula, Babil Governorate.</obo:IAO_0000115>
        <oboInOwl:hasOBONamespace>GAZ</oboInOwl:hasOBONamespace>
        <oboInOwl:id>GAZ:00251027</oboInOwl:id>
        <rdfs:label>Haur Ibn Najim</rdfs:label>
    </owl:NamedIndividual>
    


    <!-- http://purl.obolibrary.org/obo/GAZ_00251031 -->

    <owl:NamedIndividual rdf:about="http://purl.obolibrary.org/obo/GAZ_00251031">
        <obo:IAO_0000115>A canal which links the southeast corner of Haur Al Hammar to the head of the Gulf via Khawr Al Zubair.</obo:IAO_0000115>
        <oboInOwl:hasOBONamespace>GAZ</oboInOwl:hasOBONamespace>
        <oboInOwl:id>GAZ:00251031</oboInOwl:id>
        <rdfs:label>Shatt Al Basrah</rdfs:label>
    </owl:NamedIndividual>
    


    <!-- http://purl.obolibrary.org/obo/GAZ_00251032 -->

    <owl:NamedIndividual rdf:about="http://purl.obolibrary.org/obo/GAZ_00251032">
        <obo:RO_0001025 rdf:resource="http://purl.obolibrary.org/obo/GAZ_02000619"/>
        <obo:IAO_0000115>A saline lake. Located to the north of the Euphrates, about 20 km east of Samawa, Al Muthanna Governorate.</obo:IAO_0000115>
        <oboInOwl:hasOBONamespace>GAZ</oboInOwl:hasOBONamespace>
        <oboInOwl:id>GAZ:00251032</oboInOwl:id>
        <rdfs:label>Haur Lafta</rdfs:label>
    </owl:NamedIndividual>
    


    <!-- http://purl.obolibrary.org/obo/GAZ_00251033 -->

    <owl:NamedIndividual rdf:about="http://purl.obolibrary.org/obo/GAZ_00251033">
        <obo:RO_0001025 rdf:resource="http://purl.obolibrary.org/obo/GAZ_02000613"/>
        <obo:IAO_0000115>A saline wetland located to the southwest of the Tigris River about 40 km southwest of Kut, Wasit Governorate.</obo:IAO_0000115>
        <oboInOwl:hasOBONamespace>GAZ</oboInOwl:hasOBONamespace>
        <oboInOwl:id>GAZ:00251033</oboInOwl:id>
        <rdfs:label>Haur Delmaj</rdfs:label>
    </owl:NamedIndividual>
    


    <!-- http://purl.obolibrary.org/obo/GAZ_00251034 -->

    <owl:NamedIndividual rdf:about="http://purl.obolibrary.org/obo/GAZ_00251034">
        <obo:RO_0001025 rdf:resource="http://purl.obolibrary.org/obo/GAZ_02000613"/>
        <obo:IAO_0000115>A slightly brackish eutrophic lake. Located on the plain north of the Tigris River, 25 km northeast of Kut, Wasit Governorate.</obo:IAO_0000115>
        <oboInOwl:hasOBONamespace>GAZ</oboInOwl:hasOBONamespace>
        <oboInOwl:id>GAZ:00251034</oboInOwl:id>
        <rdfs:label>Haur Al Shuwaija</rdfs:label>
    </owl:NamedIndividual>
    


    <!-- http://purl.obolibrary.org/obo/GAZ_00251035 -->

    <owl:NamedIndividual rdf:about="http://purl.obolibrary.org/obo/GAZ_00251035">
        <obo:RO_0001025 rdf:resource="http://purl.obolibrary.org/obo/GAZ_02000613"/>
        <obo:IAO_0000115>A freshwater lake the plains to the east of the Shatt Al Gharraf and south of the Tigris River. Linked to the Haur Al Abjiya by the Dujaila Canal.</obo:IAO_0000115>
        <oboInOwl:hasOBONamespace>GAZ</oboInOwl:hasOBONamespace>
        <oboInOwl:id>GAZ:00251035</oboInOwl:id>
        <rdfs:label>Haur Umm Al Baram</rdfs:label>
    </owl:NamedIndividual>
    


    <!-- http://purl.obolibrary.org/obo/GAZ_00251036 -->

    <owl:NamedIndividual rdf:about="http://purl.obolibrary.org/obo/GAZ_00251036">
        <obo:RO_0001025 rdf:resource="http://purl.obolibrary.org/obo/GAZ_02000613"/>
        <obo:IAO_0000115>A freshwater lake the plains to the east of the Shatt Al Gharraf and south of the Tigris River. Linked to the Haur Umm Al Baram by the Dujaila Canal.</obo:IAO_0000115>
        <oboInOwl:hasOBONamespace>GAZ</oboInOwl:hasOBONamespace>
        <oboInOwl:id>GAZ:00251036</oboInOwl:id>
        <rdfs:label>Haur Al Abjiya</rdfs:label>
    </owl:NamedIndividual>
    


    <!-- http://purl.obolibrary.org/obo/GAZ_00251037 -->

    <owl:NamedIndividual rdf:about="http://purl.obolibrary.org/obo/GAZ_00251037">
        <obo:IAO_0000115>A canal linling Haur Umm Al Baram and Haur Al Abjiya.</obo:IAO_0000115>
        <oboInOwl:hasOBONamespace>GAZ</oboInOwl:hasOBONamespace>
        <oboInOwl:id>GAZ:00251037</oboInOwl:id>
        <rdfs:label>Dujaila Canal</rdfs:label>
    </owl:NamedIndividual>
    


    <!-- http://purl.obolibrary.org/obo/GAZ_00251038 -->

    <owl:NamedIndividual rdf:about="http://purl.obolibrary.org/obo/GAZ_00251038">
        <obo:RO_0001025 rdf:resource="http://purl.obolibrary.org/obo/GAZ_02000613"/>
        <obo:IAO_0000115>A wetland. Located on the plains to the east of the Shatt Al Gharaf, about 10 km southeast of Hai, Wasit Governorate.</obo:IAO_0000115>
        <oboInOwl:hasOBONamespace>GAZ</oboInOwl:hasOBONamespace>
        <oboInOwl:id>GAZ:00251038</oboInOwl:id>
        <rdfs:label>Haur Al Hachcham</rdfs:label>
    </owl:NamedIndividual>
    


    <!-- http://purl.obolibrary.org/obo/GAZ_00251039 -->

    <owl:NamedIndividual rdf:about="http://purl.obolibrary.org/obo/GAZ_00251039">
        <obo:RO_0001025 rdf:resource="http://purl.obolibrary.org/obo/GAZ_02000613"/>
        <obo:IAO_0000115>A wetland. Located on the plains to the east of the Shatt Al Gharaf, about 10 km southeast of Hai, Wasit Governorate.</obo:IAO_0000115>
        <oboInOwl:hasOBONamespace>GAZ</oboInOwl:hasOBONamespace>
        <oboInOwl:id>GAZ:00251039</oboInOwl:id>
        <rdfs:label>Haur Maraiba</rdfs:label>
    </owl:NamedIndividual>
    


    <!-- http://purl.obolibrary.org/obo/GAZ_00251040 -->

    <owl:NamedIndividual rdf:about="http://purl.obolibrary.org/obo/GAZ_00251040">
        <obo:RO_0001025 rdf:resource="http://purl.obolibrary.org/obo/GAZ_02000626"/>
        <obo:IAO_0000115>A wetland complex. Located on the plains to the east of the Shatt Al Gharraf, about 20 km east and southeast of Shatra, Dhi Qar Governorate.</obo:IAO_0000115>
        <oboInOwl:hasOBONamespace>GAZ</oboInOwl:hasOBONamespace>
        <oboInOwl:id>GAZ:00251040</oboInOwl:id>
        <rdfs:label>Haur Uwainah Complex</rdfs:label>
    </owl:NamedIndividual>
    


    <!-- http://purl.obolibrary.org/obo/GAZ_00251041 -->

    <owl:NamedIndividual rdf:about="http://purl.obolibrary.org/obo/GAZ_00251041">
        <obo:RO_0001025 rdf:resource="http://purl.obolibrary.org/obo/GAZ_00251040"/>
        <obo:IAO_0000115>A wetland.</obo:IAO_0000115>
        <oboInOwl:hasOBONamespace>GAZ</oboInOwl:hasOBONamespace>
        <oboInOwl:id>GAZ:00251041</oboInOwl:id>
        <rdfs:label>Haur Chamuqa</rdfs:label>
    </owl:NamedIndividual>
    


    <!-- http://purl.obolibrary.org/obo/GAZ_00251042 -->

    <owl:NamedIndividual rdf:about="http://purl.obolibrary.org/obo/GAZ_00251042">
        <obo:RO_0001025 rdf:resource="http://purl.obolibrary.org/obo/GAZ_00251040"/>
        <obo:IAO_0000115>A former wetland. Drained &lt;1972-12.</obo:IAO_0000115>
        <oboInOwl:hasOBONamespace>GAZ</oboInOwl:hasOBONamespace>
        <oboInOwl:id>GAZ:00251042</oboInOwl:id>
        <rdfs:label>Haur Abu Ajul</rdfs:label>
    </owl:NamedIndividual>
    


    <!-- http://purl.obolibrary.org/obo/GAZ_00251043 -->

    <owl:NamedIndividual rdf:about="http://purl.obolibrary.org/obo/GAZ_00251043">
        <obo:RO_0001025 rdf:resource="http://purl.obolibrary.org/obo/GAZ_02000613"/>
        <obo:IAO_0000115>A wetland. A vast shallow lake over 50 km long and covering about 1,400 km2 bordered in the east by the Tigris and in the west by the Dujaila Canal.</obo:IAO_0000115>
        <oboInOwl:hasOBONamespace>GAZ</oboInOwl:hasOBONamespace>
        <oboInOwl:id>GAZ:00251043</oboInOwl:id>
        <rdfs:label>Haur Al Sa&apos;adiyah</rdfs:label>
    </owl:NamedIndividual>
    


    <!-- http://purl.obolibrary.org/obo/GAZ_00251044 -->

    <owl:NamedIndividual rdf:about="http://purl.obolibrary.org/obo/GAZ_00251044">
        <obo:RO_0001025 rdf:resource="http://purl.obolibrary.org/obo/GAZ_00251043"/>
        <obo:IAO_0000115>A wetland.</obo:IAO_0000115>
        <oboInOwl:hasOBONamespace>GAZ</oboInOwl:hasOBONamespace>
        <oboInOwl:id>GAZ:00251044</oboInOwl:id>
        <rdfs:label>Haur Dujaila</rdfs:label>
    </owl:NamedIndividual>
    


    <!-- http://purl.obolibrary.org/obo/GAZ_00251045 -->

    <owl:NamedIndividual rdf:about="http://purl.obolibrary.org/obo/GAZ_00251045">
        <obo:RO_0001025 rdf:resource="http://purl.obolibrary.org/obo/GAZ_00251043"/>
        <obo:IAO_0000115>A wetland.</obo:IAO_0000115>
        <oboInOwl:hasOBONamespace>GAZ</oboInOwl:hasOBONamespace>
        <oboInOwl:id>GAZ:00251045</oboInOwl:id>
        <rdfs:label>Haur Umm Roij</rdfs:label>
    </owl:NamedIndividual>
    


    <!-- http://purl.obolibrary.org/obo/GAZ_00251046 -->

    <owl:NamedIndividual rdf:about="http://purl.obolibrary.org/obo/GAZ_00251046">
        <obo:RO_0001025 rdf:resource="http://purl.obolibrary.org/obo/GAZ_02000624"/>
        <obo:IAO_0000115>A wetland. Located on the east bank of the Tigris River, east and southeast of the town of Ali Gharbi, Maysan Governorate.</obo:IAO_0000115>
        <oboInOwl:hasOBONamespace>GAZ</oboInOwl:hasOBONamespace>
        <oboInOwl:id>GAZ:00251046</oboInOwl:id>
        <rdfs:label>Haur Sarut</rdfs:label>
    </owl:NamedIndividual>
    


    <!-- http://purl.obolibrary.org/obo/GAZ_00251047 -->

    <owl:NamedIndividual rdf:about="http://purl.obolibrary.org/obo/GAZ_00251047">
        <obo:RO_0001025 rdf:resource="http://purl.obolibrary.org/obo/GAZ_02000624"/>
        <obo:IAO_0000115>A wetland. Located on the east bank of the Tigris River, north of the village of Al Kumait, Maysan Governorate. It comprises a group of 14 artificial ponds (Al Kumait Ponds), constructed for wildfowl hunting, in the basin of the former Haur Al Haushiya on the east bank of the Tigris River.</obo:IAO_0000115>
        <oboInOwl:hasOBONamespace>GAZ</oboInOwl:hasOBONamespace>
        <oboInOwl:id>GAZ:00251047</oboInOwl:id>
        <rdfs:label>Haur Al Haushiya</rdfs:label>
    </owl:NamedIndividual>
    


    <!-- http://purl.obolibrary.org/obo/GAZ_00251048 -->

    <owl:NamedIndividual rdf:about="http://purl.obolibrary.org/obo/GAZ_00251048">
        <obo:RO_0001025 rdf:resource="http://purl.obolibrary.org/obo/GAZ_02000624"/>
        <obo:IAO_0000115>A wetland complex. A group of large haurs with extensive marshes on the plains to the east of the Tigris, north of Suweid Marshes. Located on the east bank of the Tigris River between Amara and Al Halfaya, about 20 km NE of Amara, Maysan Governorate.</obo:IAO_0000115>
        <oboInOwl:hasOBONamespace>GAZ</oboInOwl:hasOBONamespace>
        <oboInOwl:id>GAZ:00251048</oboInOwl:id>
        <rdfs:label>Haur Chubaisah Complex</rdfs:label>
    </owl:NamedIndividual>
    


    <!-- http://purl.obolibrary.org/obo/GAZ_00251049 -->

    <owl:NamedIndividual rdf:about="http://purl.obolibrary.org/obo/GAZ_00251049">
        <obo:RO_0001025 rdf:resource="http://purl.obolibrary.org/obo/GAZ_00251048"/>
        <obo:RO_0001025 rdf:resource="http://purl.obolibrary.org/obo/GAZ_02000624"/>
        <obo:IAO_0000115>A wetland.</obo:IAO_0000115>
        <oboInOwl:hasOBONamespace>GAZ</oboInOwl:hasOBONamespace>
        <oboInOwl:id>GAZ:00251049</oboInOwl:id>
        <rdfs:label>Haur Jazrah</rdfs:label>
    </owl:NamedIndividual>
    


    <!-- http://purl.obolibrary.org/obo/GAZ_00251050 -->

    <owl:NamedIndividual rdf:about="http://purl.obolibrary.org/obo/GAZ_00251050">
        <obo:RO_0001025 rdf:resource="http://purl.obolibrary.org/obo/GAZ_00251048"/>
        <obo:RO_0001025 rdf:resource="http://purl.obolibrary.org/obo/GAZ_02000624"/>
        <obo:IAO_0000115>A wetland.</obo:IAO_0000115>
        <oboInOwl:hasOBONamespace>GAZ</oboInOwl:hasOBONamespace>
        <oboInOwl:id>GAZ:00251050</oboInOwl:id>
        <rdfs:label>Haur Chubaisah</rdfs:label>
    </owl:NamedIndividual>
    


    <!-- http://purl.obolibrary.org/obo/GAZ_00251051 -->

    <owl:NamedIndividual rdf:about="http://purl.obolibrary.org/obo/GAZ_00251051">
        <obo:RO_0001025 rdf:resource="http://purl.obolibrary.org/obo/GAZ_00251048"/>
        <obo:RO_0001025 rdf:resource="http://purl.obolibrary.org/obo/GAZ_02000624"/>
        <obo:IAO_0000115>A wetland.</obo:IAO_0000115>
        <oboInOwl:hasOBONamespace>GAZ</oboInOwl:hasOBONamespace>
        <oboInOwl:id>GAZ:00251051</oboInOwl:id>
        <rdfs:label>Haur Sanaf</rdfs:label>
    </owl:NamedIndividual>
    


    <!-- http://purl.obolibrary.org/obo/GAZ_00251052 -->

    <owl:NamedIndividual rdf:about="http://purl.obolibrary.org/obo/GAZ_00251052">
        <obo:RO_0001025 rdf:resource="http://purl.obolibrary.org/obo/GAZ_02000624"/>
        <obo:IAO_0000115>A Canal.</obo:IAO_0000115>
        <oboInOwl:hasOBONamespace>GAZ</oboInOwl:hasOBONamespace>
        <oboInOwl:id>GAZ:00251052</oboInOwl:id>
        <rdfs:label>Musharra Canal</rdfs:label>
    </owl:NamedIndividual>
    


    <!-- http://purl.obolibrary.org/obo/GAZ_00251053 -->

    <owl:NamedIndividual rdf:about="http://purl.obolibrary.org/obo/GAZ_00251053">
        <obo:RO_0001025 rdf:resource="http://purl.obolibrary.org/obo/GAZ_02000624"/>
        <obo:IAO_0000115>A wetland. Located on the west bank of the Tigris River, 30 km west of Arnara, Maysan Governorate.</obo:IAO_0000115>
        <oboInOwl:hasOBONamespace>GAZ</oboInOwl:hasOBONamespace>
        <oboInOwl:id>GAZ:00251053</oboInOwl:id>
        <rdfs:label>Haur Sanniya</rdfs:label>
    </owl:NamedIndividual>
    


    <!-- http://purl.obolibrary.org/obo/GAZ_00251054 -->

    <owl:NamedIndividual rdf:about="http://purl.obolibrary.org/obo/GAZ_00251054">
        <obo:RO_0001025 rdf:resource="http://purl.obolibrary.org/obo/GAZ_02000624"/>
        <obo:IAO_0000115>A wetland. Located between the villages of Maymund and Salam, about 20 km SSW of Amara, Maysan Governorate.</obo:IAO_0000115>
        <oboInOwl:hasOBONamespace>GAZ</oboInOwl:hasOBONamespace>
        <oboInOwl:id>GAZ:00251054</oboInOwl:id>
        <rdfs:label>Haur Al Rayan</rdfs:label>
    </owl:NamedIndividual>
    


    <!-- http://purl.obolibrary.org/obo/GAZ_00251055 -->

    <owl:NamedIndividual rdf:about="http://purl.obolibrary.org/obo/GAZ_00251055">
        <obo:RO_0001025 rdf:resource="http://purl.obolibrary.org/obo/GAZ_00193963"/>
        <obo:IAO_0000115>A wetland. The northernmost section of the Qurna Marshes, fed by floodwaters from the Tigris.</obo:IAO_0000115>
        <oboInOwl:hasOBONamespace>GAZ</oboInOwl:hasOBONamespace>
        <oboInOwl:id>GAZ:00251055</oboInOwl:id>
        <rdfs:label>Feraigat Marshes</rdfs:label>
    </owl:NamedIndividual>
    


    <!-- http://purl.obolibrary.org/obo/GAZ_00251056 -->

    <owl:NamedIndividual rdf:about="http://purl.obolibrary.org/obo/GAZ_00251056">
        <obo:RO_0001025 rdf:resource="http://purl.obolibrary.org/obo/GAZ_02000624"/>
        <obo:IAO_0000115>A wetland. Located between the villages of Maymund and Salam, about 20 km SSW of Amara, Maysan Governorate.</obo:IAO_0000115>
        <oboInOwl:hasOBONamespace>GAZ</oboInOwl:hasOBONamespace>
        <oboInOwl:id>GAZ:00251056</oboInOwl:id>
        <rdfs:label>Haur Umm Osbah</rdfs:label>
    </owl:NamedIndividual>
    


    <!-- http://purl.obolibrary.org/obo/GAZ_00251057 -->

    <owl:NamedIndividual rdf:about="http://purl.obolibrary.org/obo/GAZ_00251057">
        <obo:RO_0001025 rdf:resource="http://purl.obolibrary.org/obo/GAZ_00251047"/>
        <obo:IAO_0000115>Man-made lakes.</obo:IAO_0000115>
        <oboInOwl:hasOBONamespace>GAZ</oboInOwl:hasOBONamespace>
        <oboInOwl:id>GAZ:00251057</oboInOwl:id>
        <rdfs:label>Al Kumait Ponds</rdfs:label>
    </owl:NamedIndividual>
    


    <!-- http://purl.obolibrary.org/obo/GAZ_00251058 -->

    <owl:NamedIndividual rdf:about="http://purl.obolibrary.org/obo/GAZ_00251058">
        <obo:RO_0001025 rdf:resource="http://purl.obolibrary.org/obo/GAZ_02000624"/>
        <obo:IAO_0000115>A distributary of the Tigris.</obo:IAO_0000115>
        <oboInOwl:hasOBONamespace>GAZ</oboInOwl:hasOBONamespace>
        <oboInOwl:id>GAZ:00251058</oboInOwl:id>
        <rdfs:label>Shatt Al Maymunah</rdfs:label>
    </owl:NamedIndividual>
    


    <!-- http://purl.obolibrary.org/obo/GAZ_00251059 -->

    <owl:NamedIndividual rdf:about="http://purl.obolibrary.org/obo/GAZ_00251059">
        <obo:RO_0001025 rdf:resource="http://purl.obolibrary.org/obo/GAZ_02000624"/>
        <obo:IAO_0000115>A wetland. Located to the west of the Shatt Al Maymunah, about 40 km southwest of Amara town.</obo:IAO_0000115>
        <oboInOwl:hasOBONamespace>GAZ</oboInOwl:hasOBONamespace>
        <oboInOwl:id>GAZ:00251059</oboInOwl:id>
        <rdfs:label>Haur Auda</rdfs:label>
    </owl:NamedIndividual>
    


    <!-- http://purl.obolibrary.org/obo/GAZ_00251060 -->

    <owl:NamedIndividual rdf:about="http://purl.obolibrary.org/obo/GAZ_00251060">
        <obo:RO_0001025 rdf:resource="http://purl.obolibrary.org/obo/GAZ_00193963"/>
        <obo:IAO_0000115>A wetland. Located in the extreme northeast of the Qurna Marshes, just west of the River Tigris.</obo:IAO_0000115>
        <oboInOwl:hasOBONamespace>GAZ</oboInOwl:hasOBONamespace>
        <oboInOwl:id>GAZ:00251060</oboInOwl:id>
        <rdfs:label>Al Azair Marshes</rdfs:label>
    </owl:NamedIndividual>
    


    <!-- http://purl.obolibrary.org/obo/GAZ_00251061 -->

    <owl:NamedIndividual rdf:about="http://purl.obolibrary.org/obo/GAZ_00251061">
        <obo:RO_0001025 rdf:resource="http://purl.obolibrary.org/obo/GAZ_00193963"/>
        <obo:IAO_0000115>A wetland surrounding Umm al Binni Lake.</obo:IAO_0000115>
        <oboInOwl:hasOBONamespace>GAZ</oboInOwl:hasOBONamespace>
        <oboInOwl:id>GAZ:00251061</oboInOwl:id>
        <rdfs:label>Haur Umm Al Binni Marshes</rdfs:label>
    </owl:NamedIndividual>
    


    <!-- http://purl.obolibrary.org/obo/GAZ_00251062 -->

    <owl:NamedIndividual rdf:about="http://purl.obolibrary.org/obo/GAZ_00251062">
        <obo:RO_0001025 rdf:resource="http://purl.obolibrary.org/obo/GAZ_00193963"/>
        <obo:IAO_0000115>A wetland. Located along western edge of the Qurna Marshes.</obo:IAO_0000115>
        <oboInOwl:hasOBONamespace>GAZ</oboInOwl:hasOBONamespace>
        <oboInOwl:id>GAZ:00251062</oboInOwl:id>
        <rdfs:label>Fartus Marshes</rdfs:label>
    </owl:NamedIndividual>
    


    <!-- http://purl.obolibrary.org/obo/GAZ_00251063 -->

    <owl:NamedIndividual rdf:about="http://purl.obolibrary.org/obo/GAZ_00251063">
        <obo:RO_0001025 rdf:resource="http://purl.obolibrary.org/obo/GAZ_00193963"/>
        <obo:IAO_0000115>A wetland. A large area of permanent and temporary marshes, including Haur Birkat (Birkat Baghdad), in the south, flooded both from the Tigris and the Euphrates.</obo:IAO_0000115>
        <oboInOwl:hasOBONamespace>GAZ</oboInOwl:hasOBONamespace>
        <oboInOwl:id>GAZ:00251063</oboInOwl:id>
        <rdfs:label>Chabaish Marshes</rdfs:label>
    </owl:NamedIndividual>
    


    <!-- http://purl.obolibrary.org/obo/GAZ_00251064 -->

    <owl:NamedIndividual rdf:about="http://purl.obolibrary.org/obo/GAZ_00251064">
        <obo:RO_0001025 rdf:resource="http://purl.obolibrary.org/obo/GAZ_00193963"/>
        <obo:IAO_0000115>A wetland. Located on the north bank of the Euphrates before its confluence with the Tigris.</obo:IAO_0000115>
        <oboInOwl:hasOBONamespace>GAZ</oboInOwl:hasOBONamespace>
        <oboInOwl:id>GAZ:00251064</oboInOwl:id>
        <rdfs:label>Al Jazair Marshes</rdfs:label>
    </owl:NamedIndividual>
    


    <!-- http://purl.obolibrary.org/obo/GAZ_00251065 -->

    <owl:NamedIndividual rdf:about="http://purl.obolibrary.org/obo/GAZ_00251065">
        <obo:RO_0001025 rdf:resource="http://purl.obolibrary.org/obo/GAZ_00251062"/>
        <oboInOwl:hasOBONamespace>GAZ</oboInOwl:hasOBONamespace>
        <oboInOwl:id>GAZ:00251065</oboInOwl:id>
        <rdfs:label>Sabil Al Awaidiya</rdfs:label>
    </owl:NamedIndividual>
    


    <!-- http://purl.obolibrary.org/obo/GAZ_00251066 -->

    <owl:NamedIndividual rdf:about="http://purl.obolibrary.org/obo/GAZ_00251066">
        <obo:RO_0001025 rdf:resource="http://purl.obolibrary.org/obo/GAZ_00251063"/>
        <obo:IAO_0000115>A wetland.</obo:IAO_0000115>
        <oboInOwl:hasOBONamespace>GAZ</oboInOwl:hasOBONamespace>
        <oboInOwl:id>GAZ:00251066</oboInOwl:id>
        <rdfs:label>Haur Birkat</rdfs:label>
    </owl:NamedIndividual>
    


    <!-- http://purl.obolibrary.org/obo/GAZ_00251067 -->

    <owl:NamedIndividual rdf:about="http://purl.obolibrary.org/obo/GAZ_00251067">
        <obo:RO_0001025 rdf:resource="http://purl.obolibrary.org/obo/GAZ_00193962"/>
        <obo:IAO_0000115>A wetland. Located in the SE of Haur Al Hammar.</obo:IAO_0000115>
        <oboInOwl:hasOBONamespace>GAZ</oboInOwl:hasOBONamespace>
        <oboInOwl:id>GAZ:00251067</oboInOwl:id>
        <rdfs:label>Haur Aluwez</rdfs:label>
    </owl:NamedIndividual>
    


    <!-- http://purl.obolibrary.org/obo/GAZ_00251068 -->

    <owl:NamedIndividual rdf:about="http://purl.obolibrary.org/obo/GAZ_00251068">
        <obo:RO_0001025 rdf:resource="http://purl.obolibrary.org/obo/GAZ_00193962"/>
        <obo:IAO_0000115>A wetland. Located in dead branches of the Euphrates at the western extremity of Haur Al Hammar near Nasiriya (Suk Al-Shiok).</obo:IAO_0000115>
        <oboInOwl:hasOBONamespace>GAZ</oboInOwl:hasOBONamespace>
        <oboInOwl:id>GAZ:00251068</oboInOwl:id>
        <rdfs:label>Nasiriya Marshes</rdfs:label>
    </owl:NamedIndividual>
    


    <!-- http://purl.obolibrary.org/obo/GAZ_00251069 -->

    <owl:NamedIndividual rdf:about="http://purl.obolibrary.org/obo/GAZ_00251069">
        <obo:RO_0001025 rdf:resource="http://purl.obolibrary.org/obo/GAZ_02000624"/>
        <obo:IAO_0000115>A large wetland on the Al Kahala (Chahala) River, about 30 km southeast of Amara.</obo:IAO_0000115>
        <oboInOwl:hasOBONamespace>GAZ</oboInOwl:hasOBONamespace>
        <oboInOwl:id>GAZ:00251069</oboInOwl:id>
        <rdfs:label>Suweid Marshes</rdfs:label>
    </owl:NamedIndividual>
    


    <!-- http://purl.obolibrary.org/obo/GAZ_00251070 -->

    <owl:NamedIndividual rdf:about="http://purl.obolibrary.org/obo/GAZ_00251070">
        <obo:RO_0001025 rdf:resource="http://purl.obolibrary.org/obo/GAZ_00193964"/>
        <obo:IAO_0000115>A wetland.</obo:IAO_0000115>
        <oboInOwl:hasOBONamespace>GAZ</oboInOwl:hasOBONamespace>
        <oboInOwl:id>GAZ:00251070</oboInOwl:id>
        <rdfs:label>Nahrsabla Marshes</rdfs:label>
    </owl:NamedIndividual>
    


    <!-- http://purl.obolibrary.org/obo/GAZ_00251071 -->

    <owl:NamedIndividual rdf:about="http://purl.obolibrary.org/obo/GAZ_00251071">
        <obo:RO_0001025 rdf:resource="http://purl.obolibrary.org/obo/GAZ_00004492"/>
        <obo:IAO_0000115>A wetland. Located from the confluence of the Tigris and Euphrates at Qurna to the head of the Gulf at Fao, Al Basrah Governorate.</obo:IAO_0000115>
        <oboInOwl:hasOBONamespace>GAZ</oboInOwl:hasOBONamespace>
        <oboInOwl:id>GAZ:00251071</oboInOwl:id>
        <rdfs:label>Shatt Al Arab Marshes</rdfs:label>
    </owl:NamedIndividual>
    


    <!-- http://purl.obolibrary.org/obo/GAZ_00251072 -->

    <owl:NamedIndividual rdf:about="http://purl.obolibrary.org/obo/GAZ_00251072">
        <obo:RO_0001025 rdf:resource="http://purl.obolibrary.org/obo/GAZ_00251071"/>
        <obo:IAO_0000115>A wetland.</obo:IAO_0000115>
        <oboInOwl:hasOBONamespace>GAZ</oboInOwl:hasOBONamespace>
        <oboInOwl:id>GAZ:00251072</oboInOwl:id>
        <rdfs:label>Haur ash Shaibah</rdfs:label>
    </owl:NamedIndividual>
    


    <!-- http://purl.obolibrary.org/obo/GAZ_00251073 -->

    <owl:NamedIndividual rdf:about="http://purl.obolibrary.org/obo/GAZ_00251073">
        <obo:RO_0001025 rdf:resource="http://purl.obolibrary.org/obo/GAZ_00251071"/>
        <obo:IAO_0000115>A wetland.</obo:IAO_0000115>
        <oboInOwl:hasOBONamespace>GAZ</oboInOwl:hasOBONamespace>
        <oboInOwl:id>GAZ:00251073</oboInOwl:id>
        <rdfs:label>Qarmat Ali Wetland</rdfs:label>
    </owl:NamedIndividual>
    


    <!-- http://purl.obolibrary.org/obo/GAZ_00251074 -->

    <owl:NamedIndividual rdf:about="http://purl.obolibrary.org/obo/GAZ_00251074">
        <obo:RO_0001025 rdf:resource="http://purl.obolibrary.org/obo/GAZ_00251071"/>
        <obo:IAO_0000115>A wetland.</obo:IAO_0000115>
        <oboInOwl:hasOBONamespace>GAZ</oboInOwl:hasOBONamespace>
        <oboInOwl:id>GAZ:00251074</oboInOwl:id>
        <rdfs:label>Khamisiyah Wetland</rdfs:label>
    </owl:NamedIndividual>
    


    <!-- http://purl.obolibrary.org/obo/GAZ_00251075 -->

    <owl:NamedIndividual rdf:about="http://purl.obolibrary.org/obo/GAZ_00251075">
        <obo:RO_0001025 rdf:resource="http://purl.obolibrary.org/obo/GAZ_00251071"/>
        <obo:IAO_0000115>A wetland.</obo:IAO_0000115>
        <oboInOwl:hasOBONamespace>GAZ</oboInOwl:hasOBONamespace>
        <oboInOwl:id>GAZ:00251075</oboInOwl:id>
        <rdfs:label>Shafi Wetland</rdfs:label>
    </owl:NamedIndividual>
    


    <!-- http://purl.obolibrary.org/obo/GAZ_00251076 -->

    <owl:NamedIndividual rdf:about="http://purl.obolibrary.org/obo/GAZ_00251076">
        <obo:IAO_0000115>A tidal inlet at the head of the Persian Gulf. It receives freshwater inflow from the Shatt Al Basrah ) at its northern end, and opens up into Khawr Abd Allah in the southeast.</obo:IAO_0000115>
        <oboInOwl:hasOBONamespace>GAZ</oboInOwl:hasOBONamespace>
        <oboInOwl:id>GAZ:00251076</oboInOwl:id>
        <rdfs:label>Khawr Al Zubair</rdfs:label>
    </owl:NamedIndividual>
    


    <!-- http://purl.obolibrary.org/obo/GAZ_00251078 -->

    <owl:NamedIndividual rdf:about="http://purl.obolibrary.org/obo/GAZ_00251078">
        <rdf:type rdf:resource="http://purl.obolibrary.org/obo/ENVO_00000004"/>
        <obo:RO_0001025 rdf:resource="http://purl.obolibrary.org/obo/GAZ_00010359"/>
        <obo:IAO_0000115>A district in Baghdad Governorate, Iraq. It is centred around the town of Al-Mahmoudiyah.</obo:IAO_0000115>
        <oboInOwl:hasOBONamespace>GAZ</oboInOwl:hasOBONamespace>
        <oboInOwl:id>GAZ:00251078</oboInOwl:id>
        <rdfs:label>Mahmudiya District</rdfs:label>
    </owl:NamedIndividual>
    


    <!-- http://purl.obolibrary.org/obo/GAZ_00251079 -->

    <owl:NamedIndividual rdf:about="http://purl.obolibrary.org/obo/GAZ_00251079">
        <rdf:type rdf:resource="http://purl.obolibrary.org/obo/ENVO_00000004"/>
        <obo:RO_0001025 rdf:resource="http://purl.obolibrary.org/obo/GAZ_00010359"/>
        <obo:IAO_0000115>A district of the Baghdad Governorate.</obo:IAO_0000115>
        <oboInOwl:hasOBONamespace>GAZ</oboInOwl:hasOBONamespace>
        <oboInOwl:id>GAZ:00251079</oboInOwl:id>
        <rdfs:label>Taji District</rdfs:label>
    </owl:NamedIndividual>
    


    <!-- http://purl.obolibrary.org/obo/GAZ_00251080 -->

    <owl:NamedIndividual rdf:about="http://purl.obolibrary.org/obo/GAZ_00251080">
        <rdf:type rdf:resource="http://purl.obolibrary.org/obo/ENVO_00000004"/>
        <obo:RO_0001025 rdf:resource="http://purl.obolibrary.org/obo/GAZ_00010359"/>
        <obo:IAO_0000115>A district of Baghdad Governorate.</obo:IAO_0000115>
        <oboInOwl:hasOBONamespace>GAZ</oboInOwl:hasOBONamespace>
        <oboInOwl:id>GAZ:00251080</oboInOwl:id>
        <rdfs:label>Al Istiqlal District</rdfs:label>
    </owl:NamedIndividual>
    


    <!-- http://purl.obolibrary.org/obo/GAZ_00251081 -->

    <owl:NamedIndividual rdf:about="http://purl.obolibrary.org/obo/GAZ_00251081">
        <rdf:type rdf:resource="http://purl.obolibrary.org/obo/ENVO_00000004"/>
        <obo:RO_0001025 rdf:resource="http://purl.obolibrary.org/obo/GAZ_00010359"/>
        <obo:IAO_0000115>A district of Baghdad Governorate.</obo:IAO_0000115>
        <oboInOwl:hasOBONamespace>GAZ</oboInOwl:hasOBONamespace>
        <oboInOwl:id>GAZ:00251081</oboInOwl:id>
        <rdfs:label>Al-Mada&apos;in District</rdfs:label>
    </owl:NamedIndividual>
    


    <!-- http://purl.obolibrary.org/obo/GAZ_00251082 -->

    <owl:NamedIndividual rdf:about="http://purl.obolibrary.org/obo/GAZ_00251082">
        <rdf:type rdf:resource="http://purl.obolibrary.org/obo/ENVO_00000004"/>
        <obo:RO_0001025 rdf:resource="http://purl.obolibrary.org/obo/GAZ_00010359"/>
        <obo:IAO_0000115>A district of Baghdad Governorate.</obo:IAO_0000115>
        <oboInOwl:hasOBONamespace>GAZ</oboInOwl:hasOBONamespace>
        <oboInOwl:id>GAZ:00251082</oboInOwl:id>
        <rdfs:label>Al Tarmia District</rdfs:label>
    </owl:NamedIndividual>
    


    <!-- http://purl.obolibrary.org/obo/GAZ_00251083 -->

    <owl:NamedIndividual rdf:about="http://purl.obolibrary.org/obo/GAZ_00251083">
        <rdf:type rdf:resource="http://purl.obolibrary.org/obo/ENVO_00000004"/>
        <obo:RO_0001025 rdf:resource="http://purl.obolibrary.org/obo/GAZ_00010359"/>
        <obo:IAO_0000115>A district of Baghdad Governorate.</obo:IAO_0000115>
        <oboInOwl:hasOBONamespace>GAZ</oboInOwl:hasOBONamespace>
        <oboInOwl:id>GAZ:00251083</oboInOwl:id>
        <rdfs:label>Baghdad City</rdfs:label>
    </owl:NamedIndividual>
    


    <!-- http://purl.obolibrary.org/obo/GAZ_00251769 -->

    <owl:NamedIndividual rdf:about="http://purl.obolibrary.org/obo/GAZ_00251769">
        <obo:RO_0001025 rdf:resource="http://purl.obolibrary.org/obo/GAZ_00018501"/>
        <obo:IAO_0000115>A shallow sea bay with inter-tidal mudflats. Located at the west end of Kuwait Bay, about 25 km west of Kuwait City centre, Al-Jahra Region.</obo:IAO_0000115>
        <oboInOwl:hasOBONamespace>GAZ</oboInOwl:hasOBONamespace>
        <oboInOwl:id>GAZ:00251769</oboInOwl:id>
        <rdfs:label>Dawhat Kazima</rdfs:label>
    </owl:NamedIndividual>
    


    <!-- http://purl.obolibrary.org/obo/GAZ_00251770 -->

    <owl:NamedIndividual rdf:about="http://purl.obolibrary.org/obo/GAZ_00251770">
        <obo:RO_0001025 rdf:resource="http://purl.obolibrary.org/obo/GAZ_00018501"/>
        <obo:IAO_0000115>A very shallow, sheltered bay on the south side of Kuwait Bay.</obo:IAO_0000115>
        <oboInOwl:hasOBONamespace>GAZ</oboInOwl:hasOBONamespace>
        <oboInOwl:id>GAZ:00251770</oboInOwl:id>
        <rdfs:label>Sulaibikhat Bay</rdfs:label>
    </owl:NamedIndividual>
    


    <!-- http://purl.obolibrary.org/obo/GAZ_00255674 -->

    <owl:NamedIndividual rdf:about="http://purl.obolibrary.org/obo/GAZ_00255674">
        <obo:RO_0001025 rdf:resource="http://purl.obolibrary.org/obo/GAZ_00005295"/>
        <obo:IAO_0000115>A bay. Located between Jubail and Abu Ali in the south-southeast and Ra&apos;s as Zawr in the northwest.</obo:IAO_0000115>
        <oboInOwl:hasOBONamespace>GAZ</oboInOwl:hasOBONamespace>
        <oboInOwl:id>GAZ:00255674</oboInOwl:id>
        <rdfs:label>Dawhat ad-Dafi</rdfs:label>
    </owl:NamedIndividual>
    


    <!-- http://purl.obolibrary.org/obo/GAZ_00255675 -->

    <owl:NamedIndividual rdf:about="http://purl.obolibrary.org/obo/GAZ_00255675">
        <obo:RO_0001025 rdf:resource="http://purl.obolibrary.org/obo/GAZ_00005295"/>
        <obo:IAO_0000115>A bay. Located between Jubail and Abu Ali in the south-southeast and Ra&apos;s as Zawr in the northwest.</obo:IAO_0000115>
        <oboInOwl:hasOBONamespace>GAZ</oboInOwl:hasOBONamespace>
        <oboInOwl:id>GAZ:00255675</oboInOwl:id>
        <rdfs:label>Dawhat al-Musallamiya</rdfs:label>
    </owl:NamedIndividual>
    


    <!-- http://purl.obolibrary.org/obo/GAZ_00255676 -->

    <owl:NamedIndividual rdf:about="http://purl.obolibrary.org/obo/GAZ_00255676">
        <obo:RO_0001025 rdf:resource="http://purl.obolibrary.org/obo/GAZ_00005295"/>
        <obo:IAO_0000115>An island. Located close to shore northeast of Jubail. Connected to the mainland north of Jubail Industrial City by causeway.</obo:IAO_0000115>
        <oboInOwl:hasOBONamespace>GAZ</oboInOwl:hasOBONamespace>
        <oboInOwl:id>GAZ:00255676</oboInOwl:id>
        <rdfs:label>Batima</rdfs:label>
    </owl:NamedIndividual>
    


    <!-- http://purl.obolibrary.org/obo/GAZ_00255677 -->

    <owl:NamedIndividual rdf:about="http://purl.obolibrary.org/obo/GAZ_00255677">
        <obo:RO_0001025 rdf:resource="http://purl.obolibrary.org/obo/GAZ_00005295"/>
        <obo:IAO_0000115>An island. Located close to shore northeast of Jubail. Connected to the mainland north of Jubail Industrial City by causeway.</obo:IAO_0000115>
        <oboInOwl:hasOBONamespace>GAZ</oboInOwl:hasOBONamespace>
        <oboInOwl:id>GAZ:00255677</oboInOwl:id>
        <rdfs:label>Abu Ali</rdfs:label>
    </owl:NamedIndividual>
    


    <!-- http://purl.obolibrary.org/obo/GAZ_00255679 -->

    <owl:NamedIndividual rdf:about="http://purl.obolibrary.org/obo/GAZ_00255679">
        <obo:RO_0001025 rdf:resource="http://purl.obolibrary.org/obo/GAZ_00005295"/>
        <obo:IAO_0000115>A group of coral islands situated about 35-90 km offshore.</obo:IAO_0000115>
        <oboInOwl:hasOBONamespace>GAZ</oboInOwl:hasOBONamespace>
        <oboInOwl:id>GAZ:00255679</oboInOwl:id>
        <rdfs:label>Gulf Coral Islands</rdfs:label>
    </owl:NamedIndividual>
    


    <!-- http://purl.obolibrary.org/obo/GAZ_00255680 -->

    <owl:NamedIndividual rdf:about="http://purl.obolibrary.org/obo/GAZ_00255680">
        <obo:RO_0001025 rdf:resource="http://purl.obolibrary.org/obo/GAZ_00255679"/>
        <obo:IAO_0000115>A coral island.</obo:IAO_0000115>
        <oboInOwl:hasOBONamespace>GAZ</oboInOwl:hasOBONamespace>
        <oboInOwl:id>GAZ:00255680</oboInOwl:id>
        <rdfs:label>Jazirat al Jurayd</rdfs:label>
    </owl:NamedIndividual>
    


    <!-- http://purl.obolibrary.org/obo/GAZ_00255681 -->

    <owl:NamedIndividual rdf:about="http://purl.obolibrary.org/obo/GAZ_00255681">
        <obo:RO_0001025 rdf:resource="http://purl.obolibrary.org/obo/GAZ_00255679"/>
        <obo:IAO_0000115>A coral island.</obo:IAO_0000115>
        <oboInOwl:hasOBONamespace>GAZ</oboInOwl:hasOBONamespace>
        <oboInOwl:id>GAZ:00255681</oboInOwl:id>
        <rdfs:label>Jazirat Karan</rdfs:label>
    </owl:NamedIndividual>
    


    <!-- http://purl.obolibrary.org/obo/GAZ_00255682 -->

    <owl:NamedIndividual rdf:about="http://purl.obolibrary.org/obo/GAZ_00255682">
        <obo:RO_0001025 rdf:resource="http://purl.obolibrary.org/obo/GAZ_00255679"/>
        <obo:IAO_0000115>A coral island.</obo:IAO_0000115>
        <oboInOwl:hasOBONamespace>GAZ</oboInOwl:hasOBONamespace>
        <oboInOwl:id>GAZ:00255682</oboInOwl:id>
        <rdfs:label>Jazirat Kurayn</rdfs:label>
    </owl:NamedIndividual>
    


    <!-- http://purl.obolibrary.org/obo/GAZ_00255683 -->

    <owl:NamedIndividual rdf:about="http://purl.obolibrary.org/obo/GAZ_00255683">
        <obo:RO_0001025 rdf:resource="http://purl.obolibrary.org/obo/GAZ_00255679"/>
        <obo:IAO_0000115>A coral island.</obo:IAO_0000115>
        <oboInOwl:hasOBONamespace>GAZ</oboInOwl:hasOBONamespace>
        <oboInOwl:id>GAZ:00255683</oboInOwl:id>
        <rdfs:label>Jazirat Jana</rdfs:label>
    </owl:NamedIndividual>
    


    <!-- http://purl.obolibrary.org/obo/GAZ_00255684 -->

    <owl:NamedIndividual rdf:about="http://purl.obolibrary.org/obo/GAZ_00255684">
        <obo:RO_0001025 rdf:resource="http://purl.obolibrary.org/obo/GAZ_00255679"/>
        <obo:IAO_0000115>A coral island.</obo:IAO_0000115>
        <oboInOwl:hasOBONamespace>GAZ</oboInOwl:hasOBONamespace>
        <oboInOwl:id>GAZ:00255684</oboInOwl:id>
        <rdfs:label>Jazirat Harqus</rdfs:label>
    </owl:NamedIndividual>
    


    <!-- http://purl.obolibrary.org/obo/GAZ_00255685 -->

    <owl:NamedIndividual rdf:about="http://purl.obolibrary.org/obo/GAZ_00255685">
        <obo:RO_0001025 rdf:resource="http://purl.obolibrary.org/obo/GAZ_00255679"/>
        <obo:IAO_0000115>A coral island.</obo:IAO_0000115>
        <oboInOwl:hasOBONamespace>GAZ</oboInOwl:hasOBONamespace>
        <oboInOwl:id>GAZ:00255685</oboInOwl:id>
        <rdfs:label>Jazirat al-Arabiyah</rdfs:label>
    </owl:NamedIndividual>
    


    <!-- http://purl.obolibrary.org/obo/GAZ_00255686 -->

    <owl:NamedIndividual rdf:about="http://purl.obolibrary.org/obo/GAZ_00255686">
        <obo:RO_0001025 rdf:resource="http://purl.obolibrary.org/obo/GAZ_00005295"/>
        <obo:IAO_0000115>A bay. Located on the Gulf coast east of Qatif and north of Dammam, Eastern Province.</obo:IAO_0000115>
        <oboInOwl:hasOBONamespace>GAZ</oboInOwl:hasOBONamespace>
        <oboInOwl:id>GAZ:00255686</oboInOwl:id>
        <rdfs:label>Tarut Bay</rdfs:label>
    </owl:NamedIndividual>
    


    <!-- http://purl.obolibrary.org/obo/GAZ_00255687 -->

    <owl:NamedIndividual rdf:about="http://purl.obolibrary.org/obo/GAZ_00255687">
        <obo:RO_0001025 rdf:resource="http://purl.obolibrary.org/obo/GAZ_00255686"/>
        <obo:IAO_0000115>An island.</obo:IAO_0000115>
        <oboInOwl:hasOBONamespace>GAZ</oboInOwl:hasOBONamespace>
        <oboInOwl:id>GAZ:00255687</oboInOwl:id>
        <rdfs:label>Za&apos;l Island</rdfs:label>
    </owl:NamedIndividual>
    


    <!-- http://purl.obolibrary.org/obo/GAZ_00255688 -->

    <owl:NamedIndividual rdf:about="http://purl.obolibrary.org/obo/GAZ_00255688">
        <obo:RO_0001025 rdf:resource="http://purl.obolibrary.org/obo/GAZ_00255686"/>
        <obo:IAO_0000115>An island. Connected to the mainland by a bridge.</obo:IAO_0000115>
        <oboInOwl:hasOBONamespace>GAZ</oboInOwl:hasOBONamespace>
        <oboInOwl:id>GAZ:00255688</oboInOwl:id>
        <rdfs:label>Tarut Island</rdfs:label>
    </owl:NamedIndividual>
    


    <!-- http://purl.obolibrary.org/obo/GAZ_00255690 -->

    <owl:NamedIndividual rdf:about="http://purl.obolibrary.org/obo/GAZ_00255690">
        <obo:RO_0001025 rdf:resource="http://purl.obolibrary.org/obo/GAZ_00005295"/>
        <obo:IAO_0000115>The gulf between the Qatar Peninsula and the mainland of Saudi Arabia.</obo:IAO_0000115>
        <oboInOwl:hasOBONamespace>GAZ</oboInOwl:hasOBONamespace>
        <oboInOwl:id>GAZ:00255690</oboInOwl:id>
        <rdfs:label>Gulf of Salwah</rdfs:label>
    </owl:NamedIndividual>
    


    <!-- http://purl.obolibrary.org/obo/GAZ_00255691 -->

    <owl:NamedIndividual rdf:about="http://purl.obolibrary.org/obo/GAZ_00255691">
        <obo:RO_0001025 rdf:resource="http://purl.obolibrary.org/obo/GAZ_00255690"/>
        <obo:IAO_0000115>An island.</obo:IAO_0000115>
        <oboInOwl:hasOBONamespace>GAZ</oboInOwl:hasOBONamespace>
        <oboInOwl:id>GAZ:00255691</oboInOwl:id>
        <rdfs:label>Jazirat az Zakhnuniyah</rdfs:label>
    </owl:NamedIndividual>
    


    <!-- http://purl.obolibrary.org/obo/GAZ_00255692 -->

    <owl:NamedIndividual rdf:about="http://purl.obolibrary.org/obo/GAZ_00255692">
        <obo:RO_0001025 rdf:resource="http://purl.obolibrary.org/obo/GAZ_00255690"/>
        <obo:IAO_0000115>An island.</obo:IAO_0000115>
        <oboInOwl:hasOBONamespace>GAZ</oboInOwl:hasOBONamespace>
        <oboInOwl:id>GAZ:00255692</oboInOwl:id>
        <rdfs:label>Judhaim Island</rdfs:label>
    </owl:NamedIndividual>
    


    <!-- http://purl.obolibrary.org/obo/GAZ_00255693 -->

    <owl:NamedIndividual rdf:about="http://purl.obolibrary.org/obo/GAZ_00255693">
        <obo:RO_0001025 rdf:resource="http://purl.obolibrary.org/obo/GAZ_00255690"/>
        <obo:IAO_0000115>An island.</obo:IAO_0000115>
        <oboInOwl:hasOBONamespace>GAZ</oboInOwl:hasOBONamespace>
        <oboInOwl:id>GAZ:00255693</oboInOwl:id>
        <rdfs:label>Samamik Island</rdfs:label>
    </owl:NamedIndividual>
    


    <!-- http://purl.obolibrary.org/obo/GAZ_00255694 -->

    <owl:NamedIndividual rdf:about="http://purl.obolibrary.org/obo/GAZ_00255694">
        <obo:RO_0001025 rdf:resource="http://purl.obolibrary.org/obo/GAZ_00255690"/>
        <obo:IAO_0000115>An island.</obo:IAO_0000115>
        <oboInOwl:hasOBONamespace>GAZ</oboInOwl:hasOBONamespace>
        <oboInOwl:id>GAZ:00255694</oboInOwl:id>
        <rdfs:label>Unaibir Island</rdfs:label>
    </owl:NamedIndividual>
    


    <!-- http://purl.obolibrary.org/obo/GAZ_00256561 -->

    <owl:NamedIndividual rdf:about="http://purl.obolibrary.org/obo/GAZ_00256561">
        <obo:IAO_0000115>A low-lying island in the middle of the Euphrates.</obo:IAO_0000115>
        <oboInOwl:hasOBONamespace>GAZ</oboInOwl:hasOBONamespace>
        <oboInOwl:id>GAZ:00256561</oboInOwl:id>
        <rdfs:label>Huwaijat al-Mayadin</rdfs:label>
    </owl:NamedIndividual>
    


    <!-- http://purl.obolibrary.org/obo/GAZ_00256563 -->

    <owl:NamedIndividual rdf:about="http://purl.obolibrary.org/obo/GAZ_00256563">
        <obo:RO_0001025 rdf:resource="http://purl.obolibrary.org/obo/GAZ_00062456"/>
        <obo:IAO_0000115>An island.</obo:IAO_0000115>
        <oboInOwl:hasOBONamespace>GAZ</oboInOwl:hasOBONamespace>
        <oboInOwl:id>GAZ:00256563</oboInOwl:id>
        <rdfs:label>Jazirat al-&apos;Ayd</rdfs:label>
    </owl:NamedIndividual>
    


    <!-- http://purl.obolibrary.org/obo/GAZ_00256564 -->

    <owl:NamedIndividual rdf:about="http://purl.obolibrary.org/obo/GAZ_00256564">
        <obo:IAO_0000115>A water storage resevoir. Formed by a dam on the Euphrates at Mansurah, 10 km downstream from the main dam of Buhayrat al-Asad at Al-Thawra.</obo:IAO_0000115>
        <oboInOwl:hasOBONamespace>GAZ</oboInOwl:hasOBONamespace>
        <oboInOwl:id>GAZ:00256564</oboInOwl:id>
        <rdfs:label>Baath Lake</rdfs:label>
    </owl:NamedIndividual>
    


    <!-- http://purl.obolibrary.org/obo/GAZ_00256566 -->

    <owl:NamedIndividual rdf:about="http://purl.obolibrary.org/obo/GAZ_00256566">
        <obo:IAO_0000115>A seasonally flooded saline lake in the Syrian Desert. Located several km south and southeast of Tadmur (Palmyra), Homs Governorate.</obo:IAO_0000115>
        <oboInOwl:hasOBONamespace>GAZ</oboInOwl:hasOBONamespace>
        <oboInOwl:id>GAZ:00256566</oboInOwl:id>
        <rdfs:label>Sabkhat Muh</rdfs:label>
    </owl:NamedIndividual>
    


    <!-- http://purl.obolibrary.org/obo/GAZ_00256583 -->

    <owl:NamedIndividual rdf:about="http://purl.obolibrary.org/obo/GAZ_00256583">
        <obo:IAO_0000115>A river.</obo:IAO_0000115>
        <oboInOwl:hasOBONamespace>GAZ</oboInOwl:hasOBONamespace>
        <oboInOwl:id>GAZ:00256583</oboInOwl:id>
        <rdfs:label>Wadi Khnezir</rdfs:label>
    </owl:NamedIndividual>
    


    <!-- http://purl.obolibrary.org/obo/GAZ_00256584 -->

    <owl:NamedIndividual rdf:about="http://purl.obolibrary.org/obo/GAZ_00256584">
        <obo:IAO_0000115>A river.</obo:IAO_0000115>
        <oboInOwl:hasOBONamespace>GAZ</oboInOwl:hasOBONamespace>
        <oboInOwl:id>GAZ:00256584</oboInOwl:id>
        <rdfs:label>Wadi Jarrah</rdfs:label>
    </owl:NamedIndividual>
    


    <!-- http://purl.obolibrary.org/obo/GAZ_00256585 -->

    <owl:NamedIndividual rdf:about="http://purl.obolibrary.org/obo/GAZ_00256585">
        <obo:IAO_0000115>A river.</obo:IAO_0000115>
        <oboInOwl:hasOBONamespace>GAZ</oboInOwl:hasOBONamespace>
        <oboInOwl:id>GAZ:00256585</oboInOwl:id>
        <rdfs:label>Wadi Khanzir</rdfs:label>
    </owl:NamedIndividual>
    


    <!-- http://purl.obolibrary.org/obo/GAZ_00256607 -->

    <owl:NamedIndividual rdf:about="http://purl.obolibrary.org/obo/GAZ_00256607">
        <obo:RO_0001025 rdf:resource="http://purl.obolibrary.org/obo/GAZ_00256563"/>
        <obo:IAO_0000115>A protected area. Established 1994.</obo:IAO_0000115>
        <oboInOwl:hasOBONamespace>GAZ</oboInOwl:hasOBONamespace>
        <oboInOwl:id>GAZ:00256607</oboInOwl:id>
        <rdfs:label>Al - Thawra Protected Area</rdfs:label>
    </owl:NamedIndividual>
    


    <!-- http://purl.obolibrary.org/obo/GAZ_02000358 -->

    <owl:NamedIndividual rdf:about="http://purl.obolibrary.org/obo/GAZ_02000358"/>
    


    <!-- http://purl.obolibrary.org/obo/GAZ_02000359 -->

    <owl:NamedIndividual rdf:about="http://purl.obolibrary.org/obo/GAZ_02000359">
        <obo:RO_0001025 rdf:resource="http://purl.obolibrary.org/obo/GAZ_00006938"/>
    </owl:NamedIndividual>
    


    <!-- http://purl.obolibrary.org/obo/GAZ_02000360 -->

    <owl:NamedIndividual rdf:about="http://purl.obolibrary.org/obo/GAZ_02000360"/>
    


    <!-- http://purl.obolibrary.org/obo/GAZ_02000361 -->

    <owl:NamedIndividual rdf:about="http://purl.obolibrary.org/obo/GAZ_02000361"/>
    


    <!-- http://purl.obolibrary.org/obo/GAZ_02000362 -->

    <owl:NamedIndividual rdf:about="http://purl.obolibrary.org/obo/GAZ_02000362"/>
    


    <!-- http://purl.obolibrary.org/obo/GAZ_02000613 -->

    <owl:NamedIndividual rdf:about="http://purl.obolibrary.org/obo/GAZ_02000613"/>
    


    <!-- http://purl.obolibrary.org/obo/GAZ_02000614 -->

    <owl:NamedIndividual rdf:about="http://purl.obolibrary.org/obo/GAZ_02000614"/>
    


    <!-- http://purl.obolibrary.org/obo/GAZ_02000615 -->

    <owl:NamedIndividual rdf:about="http://purl.obolibrary.org/obo/GAZ_02000615">
        <obo:RO_0001025 rdf:resource="http://purl.obolibrary.org/obo/GAZ_00057476"/>
    </owl:NamedIndividual>
    


    <!-- http://purl.obolibrary.org/obo/GAZ_02000616 -->

    <owl:NamedIndividual rdf:about="http://purl.obolibrary.org/obo/GAZ_02000616"/>
    


    <!-- http://purl.obolibrary.org/obo/GAZ_02000617 -->

    <owl:NamedIndividual rdf:about="http://purl.obolibrary.org/obo/GAZ_02000617">
        <obo:RO_0001025 rdf:resource="http://purl.obolibrary.org/obo/GAZ_00057476"/>
    </owl:NamedIndividual>
    


    <!-- http://purl.obolibrary.org/obo/GAZ_02000618 -->

    <owl:NamedIndividual rdf:about="http://purl.obolibrary.org/obo/GAZ_02000618"/>
    


    <!-- http://purl.obolibrary.org/obo/GAZ_02000619 -->

    <owl:NamedIndividual rdf:about="http://purl.obolibrary.org/obo/GAZ_02000619"/>
    


    <!-- http://purl.obolibrary.org/obo/GAZ_02000620 -->

    <owl:NamedIndividual rdf:about="http://purl.obolibrary.org/obo/GAZ_02000620"/>
    


    <!-- http://purl.obolibrary.org/obo/GAZ_02000621 -->

    <owl:NamedIndividual rdf:about="http://purl.obolibrary.org/obo/GAZ_02000621"/>
    


    <!-- http://purl.obolibrary.org/obo/GAZ_02000622 -->

    <owl:NamedIndividual rdf:about="http://purl.obolibrary.org/obo/GAZ_02000622"/>
    


    <!-- http://purl.obolibrary.org/obo/GAZ_02000623 -->

    <owl:NamedIndividual rdf:about="http://purl.obolibrary.org/obo/GAZ_02000623"/>
    


    <!-- http://purl.obolibrary.org/obo/GAZ_02000624 -->

    <owl:NamedIndividual rdf:about="http://purl.obolibrary.org/obo/GAZ_02000624"/>
    


    <!-- http://purl.obolibrary.org/obo/GAZ_02000625 -->

    <owl:NamedIndividual rdf:about="http://purl.obolibrary.org/obo/GAZ_02000625"/>
    


    <!-- http://purl.obolibrary.org/obo/GAZ_02000626 -->

    <owl:NamedIndividual rdf:about="http://purl.obolibrary.org/obo/GAZ_02000626"/>
    


    <!-- http://purl.obolibrary.org/obo/GAZ_02000627 -->

    <owl:NamedIndividual rdf:about="http://purl.obolibrary.org/obo/GAZ_02000627"/>
    


    <!-- 
    ///////////////////////////////////////////////////////////////////////////////////////
    //
    // Annotations
    //
    ///////////////////////////////////////////////////////////////////////////////////////
     -->

    <rdf:Description rdf:about="http://purl.obolibrary.org/obo/GAZ_00004491">
        <oboInOwl:id>GAZ:00004491</oboInOwl:id>
        <oboInOwl:hasOBONamespace>GAZ</oboInOwl:hasOBONamespace>
        <rdfs:label>Governorate (Iraq)</rdfs:label>
    </rdf:Description>
    <rdf:Description rdf:about="http://purl.obolibrary.org/obo/GAZ_00004492">
        <obo:IAO_0000115>A province in southern Iraq bordering Kuwait to the south and Iran to the east.</obo:IAO_0000115>
        <oboInOwl:id>GAZ:00004492</oboInOwl:id>
        <oboInOwl:hasOBONamespace>GAZ</oboInOwl:hasOBONamespace>
        <rdfs:label>Al Basra Governorate</rdfs:label>
    </rdf:Description>
    <rdf:Description rdf:about="http://purl.obolibrary.org/obo/GAZ_00004493">
        <oboInOwl:id>GAZ:00004493</oboInOwl:id>
        <rdfs:label>Basra</rdfs:label>
        <oboInOwl:hasOBONamespace>GAZ</oboInOwl:hasOBONamespace>
    </rdf:Description>
    <rdf:Description rdf:about="http://purl.obolibrary.org/obo/GAZ_00004495">
        <rdfs:label>populated place, Iraq</rdfs:label>
        <oboInOwl:hasOBONamespace>GAZ</oboInOwl:hasOBONamespace>
        <oboInOwl:id>GAZ:00004495</oboInOwl:id>
    </rdf:Description>
    <rdf:Description rdf:about="http://purl.obolibrary.org/obo/GAZ_00009519">
        <oboInOwl:id>GAZ:00009519</oboInOwl:id>
        <rdfs:label>Governorate (Bahrain)</rdfs:label>
        <oboInOwl:hasOBONamespace>GAZ</oboInOwl:hasOBONamespace>
    </rdf:Description>
    <rdf:Description rdf:about="http://purl.obolibrary.org/obo/GAZ_00010359">
        <oboInOwl:id>GAZ:00010359</oboInOwl:id>
        <rdfs:label>Baghdad Governorate</rdfs:label>
        <oboInOwl:hasOBONamespace>GAZ</oboInOwl:hasOBONamespace>
        <obo:IAO_0000115>A governorate in the nation of Iraq includes the city of Baghdad and the surrounding metropolitan area, including Al Mahmudiyah. It has an area of 734 km2 the smallest of the 18 governorates of Iraq but the most populous.</obo:IAO_0000115>
    </rdf:Description>
    <rdf:Description rdf:about="http://purl.obolibrary.org/obo/GAZ_00010360">
        <oboInOwl:hasOBONamespace>GAZ</oboInOwl:hasOBONamespace>
        <oboInOwl:id>GAZ:00010360</oboInOwl:id>
        <rdfs:label>Baghdad</rdfs:label>
    </rdf:Description>
    <rdf:Description rdf:about="http://purl.obolibrary.org/obo/GAZ_00030835">
        <rdfs:label>Ninawa Governorate</rdfs:label>
        <obo:IAO_0000115>One of the governorates of Iraq.</obo:IAO_0000115>
        <oboInOwl:id>GAZ:00030835</oboInOwl:id>
        <oboInOwl:hasOBONamespace>GAZ</oboInOwl:hasOBONamespace>
    </rdf:Description>
    <rdf:Description rdf:about="http://purl.obolibrary.org/obo/GAZ_00052482">
        <oboInOwl:hasOBONamespace>GAZ</oboInOwl:hasOBONamespace>
        <rdfs:label>Sulaymaniyah</rdfs:label>
        <obo:IAO_0000115>A populated place. A city in the east of Iraqi Kurdistan.</obo:IAO_0000115>
        <oboInOwl:id>GAZ:00052482</oboInOwl:id>
    </rdf:Description>
    <rdf:Description rdf:about="http://purl.obolibrary.org/obo/GAZ_00052483">
        <obo:IAO_0000115>A populated place. A city in northern Iraq.</obo:IAO_0000115>
        <oboInOwl:hasOBONamespace>GAZ</oboInOwl:hasOBONamespace>
        <rdfs:label>Dahuk</rdfs:label>
        <oboInOwl:id>GAZ:00052483</oboInOwl:id>
    </rdf:Description>
    <rdf:Description rdf:about="http://purl.obolibrary.org/obo/GAZ_00052484">
        <oboInOwl:id>GAZ:00052484</oboInOwl:id>
        <oboInOwl:hasOBONamespace>GAZ</oboInOwl:hasOBONamespace>
        <obo:IAO_0000115>A populated place. A city in the Iraqi province of Al Anbar, located roughly 69 km W of Baghdad on the Euphrates.</obo:IAO_0000115>
        <rdfs:label>Fallujah</rdfs:label>
    </rdf:Description>
    <rdf:Description rdf:about="http://purl.obolibrary.org/obo/GAZ_00052486">
        <obo:IAO_0000115>A populated place. located in the sub-district of Soran, Iraq close to the Iranian border.</obo:IAO_0000115>
        <oboInOwl:id>GAZ:00052486</oboInOwl:id>
        <oboInOwl:hasOBONamespace>GAZ</oboInOwl:hasOBONamespace>
        <rdfs:label>Rowanduz</rdfs:label>
    </rdf:Description>
    <rdf:Description rdf:about="http://purl.obolibrary.org/obo/GAZ_00052487">
        <oboInOwl:id>GAZ:00052487</oboInOwl:id>
        <oboInOwl:hasOBONamespace>GAZ</oboInOwl:hasOBONamespace>
        <rdfs:label>Shaqlawa</rdfs:label>
    </rdf:Description>
    <rdf:Description rdf:about="http://purl.obolibrary.org/obo/GAZ_00052488">
        <oboInOwl:id>GAZ:00052488</oboInOwl:id>
        <oboInOwl:hasOBONamespace>GAZ</oboInOwl:hasOBONamespace>
        <rdfs:label>Zawita-i-Zheri</rdfs:label>
        <obo:IAO_0000115>A populated place.</obo:IAO_0000115>
    </rdf:Description>
    <rdf:Description rdf:about="http://purl.obolibrary.org/obo/GAZ_00053729">
        <oboInOwl:id>GAZ:00053729</oboInOwl:id>
        <oboInOwl:hasOBONamespace>GAZ</oboInOwl:hasOBONamespace>
        <obo:IAO_0000115>A populated place. A city in the Khuzestan province in southwestern Iran, located on Abadan Island.</obo:IAO_0000115>
        <rdfs:label>Abadan</rdfs:label>
    </rdf:Description>
    <rdf:Description rdf:about="http://purl.obolibrary.org/obo/GAZ_02000358">
        <oboInOwl:id>GAZ:02000358</oboInOwl:id>
        <obo:IAO_0000115>The largest of the five governorates of Bahrain.</obo:IAO_0000115>
        <oboInOwl:hasOBONamespace>GAZ</oboInOwl:hasOBONamespace>
        <rdfs:label>Southern Governorate</rdfs:label>
    </rdf:Description>
    <rdf:Description rdf:about="http://purl.obolibrary.org/obo/GAZ_02000359">
        <oboInOwl:id>GAZ:02000359</oboInOwl:id>
        <rdfs:label>Al Muharraq Governorate</rdfs:label>
        <obo:IAO_0000115>One of the five governorates of Bahrain.</obo:IAO_0000115>
        <oboInOwl:hasOBONamespace>GAZ</oboInOwl:hasOBONamespace>
    </rdf:Description>
    <rdf:Description rdf:about="http://purl.obolibrary.org/obo/GAZ_02000360">
        <rdfs:label>Northern Governorate</rdfs:label>
        <oboInOwl:hasOBONamespace>GAZ</oboInOwl:hasOBONamespace>
        <obo:IAO_0000115>One of the five governorates of Bahrain.</obo:IAO_0000115>
        <oboInOwl:id>GAZ:02000360</oboInOwl:id>
    </rdf:Description>
    <rdf:Description rdf:about="http://purl.obolibrary.org/obo/GAZ_02000361">
        <rdfs:label>Central Governorate</rdfs:label>
        <oboInOwl:hasOBONamespace>GAZ</oboInOwl:hasOBONamespace>
        <oboInOwl:id>GAZ:02000361</oboInOwl:id>
        <obo:IAO_0000115>One of the five governorates of Bahrain.</obo:IAO_0000115>
    </rdf:Description>
    <rdf:Description rdf:about="http://purl.obolibrary.org/obo/GAZ_02000362">
        <rdfs:label>Capital Governorate</rdfs:label>
        <oboInOwl:hasOBONamespace>GAZ</oboInOwl:hasOBONamespace>
        <oboInOwl:id>GAZ:02000362</oboInOwl:id>
        <obo:IAO_0000115>One of the five governorates of Bahrain.</obo:IAO_0000115>
    </rdf:Description>
    <rdf:Description rdf:about="http://purl.obolibrary.org/obo/GAZ_02000613">
        <obo:IAO_0000115>One of the governorates of Iraq. It is in the east of the country.</obo:IAO_0000115>
        <oboInOwl:id>GAZ:02000613</oboInOwl:id>
        <oboInOwl:hasOBONamespace>GAZ</oboInOwl:hasOBONamespace>
        <rdfs:label>Wasit Governorate</rdfs:label>
    </rdf:Description>
    <rdf:Description rdf:about="http://purl.obolibrary.org/obo/GAZ_02000614">
        <rdfs:label>Karbala Governorate</rdfs:label>
        <oboInOwl:hasOBONamespace>GAZ</oboInOwl:hasOBONamespace>
        <oboInOwl:id>GAZ:02000614</oboInOwl:id>
        <obo:IAO_0000115>A province in the central region of Iraq comprised of 3 districts.</obo:IAO_0000115>
    </rdf:Description>
    <rdf:Description rdf:about="http://purl.obolibrary.org/obo/GAZ_02000615">
        <oboInOwl:hasOBONamespace>GAZ</oboInOwl:hasOBONamespace>
        <oboInOwl:id>GAZ:02000615</oboInOwl:id>
        <rdfs:label>As-Sulaymaniyah Governorate</rdfs:label>
        <obo:IAO_0000115>A governorate of Iraq, within the Iraqi Kurdistan Region. Its capital is a city of the same name, As Sulaymaniyah.</obo:IAO_0000115>
    </rdf:Description>
    <rdf:Description rdf:about="http://purl.obolibrary.org/obo/GAZ_02000616">
        <oboInOwl:hasOBONamespace>GAZ</oboInOwl:hasOBONamespace>
        <rdfs:label>Salah ad-Din Governorate</rdfs:label>
        <oboInOwl:id>GAZ:02000616</oboInOwl:id>
        <obo:IAO_0000115>A governorate in Iraq, north of Baghdad. Before 1976 the governorate was part of Baghdad Governorate.</obo:IAO_0000115>
    </rdf:Description>
    <rdf:Description rdf:about="http://purl.obolibrary.org/obo/GAZ_02000617">
        <oboInOwl:hasOBONamespace>GAZ</oboInOwl:hasOBONamespace>
        <rdfs:label>Arbil Governorate</rdfs:label>
        <obo:IAO_0000115>A governorate of Iraq located in the north of the country.</obo:IAO_0000115>
        <oboInOwl:id>GAZ:02000617</oboInOwl:id>
    </rdf:Description>
    <rdf:Description rdf:about="http://purl.obolibrary.org/obo/GAZ_02000618">
        <oboInOwl:hasOBONamespace>GAZ</oboInOwl:hasOBONamespace>
        <oboInOwl:id>GAZ:02000618</oboInOwl:id>
        <rdfs:label>An-Najaf Governorate</rdfs:label>
        <obo:IAO_0000115>A province in the nation of Iraq.</obo:IAO_0000115>
    </rdf:Description>
    <rdf:Description rdf:about="http://purl.obolibrary.org/obo/GAZ_02000619">
        <oboInOwl:hasOBONamespace>GAZ</oboInOwl:hasOBONamespace>
        <rdfs:label>Al-Muthanna Governorate</rdfs:label>
        <oboInOwl:id>GAZ:02000619</oboInOwl:id>
        <obo:IAO_0000115>One of the governorates of Iraq. It is in the south of the country, bordering Saudi Arabia.</obo:IAO_0000115>
    </rdf:Description>
    <rdf:Description rdf:about="http://purl.obolibrary.org/obo/GAZ_02000620">
        <oboInOwl:id>GAZ:02000620</oboInOwl:id>
        <obo:IAO_0000115>One of the constituent governorates of the nation of Iraq. Diyala province extends to the northeast of Baghdad as far as the Iranian border. Its capital is Baqubah. It covers an area of 17,685 km2.</obo:IAO_0000115>
        <oboInOwl:hasOBONamespace>GAZ</oboInOwl:hasOBONamespace>
        <rdfs:label>Diyala Governorate</rdfs:label>
    </rdf:Description>
    <rdf:Description rdf:about="http://purl.obolibrary.org/obo/GAZ_02000621">
        <oboInOwl:hasOBONamespace>GAZ</oboInOwl:hasOBONamespace>
        <oboInOwl:id>GAZ:02000621</oboInOwl:id>
        <obo:IAO_0000115>One of the Governorates of Iraq located in the north of the country.</obo:IAO_0000115>
        <rdfs:label>Kirkuk Governorate</rdfs:label>
    </rdf:Description>
    <rdf:Description rdf:about="http://purl.obolibrary.org/obo/GAZ_02000622">
        <oboInOwl:hasOBONamespace>GAZ</oboInOwl:hasOBONamespace>
        <rdfs:label>Babil Governorate</rdfs:label>
        <oboInOwl:id>GAZ:02000622</oboInOwl:id>
        <obo:IAO_0000115>A province in central Iraq.</obo:IAO_0000115>
    </rdf:Description>
    <rdf:Description rdf:about="http://purl.obolibrary.org/obo/GAZ_02000623">
        <oboInOwl:id>GAZ:02000623</oboInOwl:id>
        <oboInOwl:hasOBONamespace>GAZ</oboInOwl:hasOBONamespace>
        <rdfs:label>Al-Qadisiyah Governorate</rdfs:label>
        <obo:IAO_0000115>One of the provinces of Iraq. It is in the center of the country. Its capital is ad-Diwaniyyah.</obo:IAO_0000115>
    </rdf:Description>
    <rdf:Description rdf:about="http://purl.obolibrary.org/obo/GAZ_02000624">
        <rdfs:label>Maysan Governorate</rdfs:label>
        <oboInOwl:id>GAZ:02000624</oboInOwl:id>
        <oboInOwl:hasOBONamespace>GAZ</oboInOwl:hasOBONamespace>
        <obo:IAO_0000115>A Governorate in southeastern Iraq, bordering Iran. The provincial capital, located beside the Tigris, is Al Amarah.</obo:IAO_0000115>
    </rdf:Description>
    <rdf:Description rdf:about="http://purl.obolibrary.org/obo/GAZ_02000625">
        <obo:IAO_0000115>One of the governorates of Iraq. It is in the north of the country. Its capital is Duhok city.</obo:IAO_0000115>
        <rdfs:label>Dahuk Governorate</rdfs:label>
        <oboInOwl:hasOBONamespace>GAZ</oboInOwl:hasOBONamespace>
        <oboInOwl:id>GAZ:02000625</oboInOwl:id>
    </rdf:Description>
    <rdf:Description rdf:about="http://purl.obolibrary.org/obo/GAZ_02000626">
        <obo:IAO_0000115>A Governorate in southern Iraq.</obo:IAO_0000115>
        <oboInOwl:hasOBONamespace>GAZ</oboInOwl:hasOBONamespace>
        <rdfs:label>Dhi Qar Governorate</rdfs:label>
        <oboInOwl:id>GAZ:02000626</oboInOwl:id>
    </rdf:Description>
    <rdf:Description rdf:about="http://purl.obolibrary.org/obo/GAZ_02000627">
        <oboInOwl:hasOBONamespace>GAZ</oboInOwl:hasOBONamespace>
        <rdfs:label>Al-Anbar Governorate</rdfs:label>
        <obo:IAO_0000115>A governorate of Iraq. Tt has shares borders with Syria, Jordan, and Saudi Arabia. Its capital is Ar Ramadi.</obo:IAO_0000115>
        <oboInOwl:id>GAZ:02000627</oboInOwl:id>
    </rdf:Description>
</rdf:RDF>



<!-- Generated by the OWL API (version 4.5.6) https://github.com/owlcs/owlapi -->

