<?xml version="1.0"?>
<rdf:RDF xmlns="http://purl.obolibrary.org/obo/gaz/subsets/countries/Israel.owl#"
     xml:base="http://purl.obolibrary.org/obo/gaz/subsets/countries/Israel.owl"
     xmlns:obo="http://purl.obolibrary.org/obo/"
     xmlns:owl="http://www.w3.org/2002/07/owl#"
     xmlns:rdf="http://www.w3.org/1999/02/22-rdf-syntax-ns#"
     xmlns:xml="http://www.w3.org/XML/1998/namespace"
     xmlns:xsd="http://www.w3.org/2001/XMLSchema#"
     xmlns:rdfs="http://www.w3.org/2000/01/rdf-schema#"
     xmlns:oboInOwl="http://www.geneontology.org/formats/oboInOwl#">
    <owl:Ontology rdf:about="http://purl.obolibrary.org/obo/gaz/subsets/countries/Israel.owl">
        <owl:imports rdf:resource="http://purl.obolibrary.org/obo/gaz/imports/envo_import.owl"/>
        <owl:imports rdf:resource="http://purl.obolibrary.org/obo/gaz/imports/ro_import.owl"/>
    </owl:Ontology>
    


    <!-- 
    ///////////////////////////////////////////////////////////////////////////////////////
    //
    // Annotation properties
    //
    ///////////////////////////////////////////////////////////////////////////////////////
     -->

    


    <!-- http://purl.obolibrary.org/obo/IAO_0000115 -->

    <owl:AnnotationProperty rdf:about="http://purl.obolibrary.org/obo/IAO_0000115"/>
    


    <!-- http://www.geneontology.org/formats/oboInOwl#hasOBONamespace -->

    <owl:AnnotationProperty rdf:about="http://www.geneontology.org/formats/oboInOwl#hasOBONamespace"/>
    


    <!-- http://www.geneontology.org/formats/oboInOwl#id -->

    <owl:AnnotationProperty rdf:about="http://www.geneontology.org/formats/oboInOwl#id"/>
    


    <!-- 
    ///////////////////////////////////////////////////////////////////////////////////////
    //
    // Object Properties
    //
    ///////////////////////////////////////////////////////////////////////////////////////
     -->

    


    <!-- http://purl.obolibrary.org/obo/RO_0001025 -->

    <owl:ObjectProperty rdf:about="http://purl.obolibrary.org/obo/RO_0001025"/>
    


    <!-- 
    ///////////////////////////////////////////////////////////////////////////////////////
    //
    // Classes
    //
    ///////////////////////////////////////////////////////////////////////////////////////
     -->

    


    <!-- http://purl.obolibrary.org/obo/ENVO_00000009 -->

    <owl:Class rdf:about="http://purl.obolibrary.org/obo/ENVO_00000009"/>
    


    <!-- http://purl.obolibrary.org/obo/ENVO_00000032 -->

    <owl:Class rdf:about="http://purl.obolibrary.org/obo/ENVO_00000032"/>
    


    <!-- http://purl.obolibrary.org/obo/ENVO_00000062 -->

    <owl:Class rdf:about="http://purl.obolibrary.org/obo/ENVO_00000062"/>
    


    <!-- http://purl.obolibrary.org/obo/ENVO_00000856 -->

    <owl:Class rdf:about="http://purl.obolibrary.org/obo/ENVO_00000856"/>
    


    <!-- http://purl.obolibrary.org/obo/GAZ_00002705 -->

    <owl:Class rdf:about="http://purl.obolibrary.org/obo/GAZ_00002705"/>
    


    <!-- http://purl.obolibrary.org/obo/GAZ_00002706 -->

    <owl:Class rdf:about="http://purl.obolibrary.org/obo/GAZ_00002706">
        <rdfs:subClassOf rdf:resource="http://purl.obolibrary.org/obo/GAZ_00002705"/>
    </owl:Class>
    


    <!-- http://purl.obolibrary.org/obo/GAZ_00002707 -->

    <owl:Class rdf:about="http://purl.obolibrary.org/obo/GAZ_00002707"/>
    


    <!-- http://purl.obolibrary.org/obo/GAZ_00002708 -->

    <owl:Class rdf:about="http://purl.obolibrary.org/obo/GAZ_00002708">
        <rdfs:subClassOf rdf:resource="http://purl.obolibrary.org/obo/GAZ_00002707"/>
    </owl:Class>
    


    <!-- http://purl.obolibrary.org/obo/GAZ_00002709 -->

    <owl:Class rdf:about="http://purl.obolibrary.org/obo/GAZ_00002709">
        <rdfs:subClassOf rdf:resource="http://purl.obolibrary.org/obo/GAZ_00002707"/>
    </owl:Class>
    


    <!-- http://purl.obolibrary.org/obo/GAZ_00002710 -->

    <owl:Class rdf:about="http://purl.obolibrary.org/obo/GAZ_00002710">
        <rdfs:subClassOf rdf:resource="http://purl.obolibrary.org/obo/GAZ_00002707"/>
    </owl:Class>
    


    <!-- http://purl.obolibrary.org/obo/GAZ_00002711 -->

    <owl:Class rdf:about="http://purl.obolibrary.org/obo/GAZ_00002711">
        <rdfs:subClassOf rdf:resource="http://purl.obolibrary.org/obo/GAZ_00002707"/>
    </owl:Class>
    


    <!-- http://purl.obolibrary.org/obo/GAZ_00002712 -->

    <owl:Class rdf:about="http://purl.obolibrary.org/obo/GAZ_00002712">
        <rdfs:subClassOf rdf:resource="http://purl.obolibrary.org/obo/GAZ_00002707"/>
    </owl:Class>
    


    <!-- http://purl.obolibrary.org/obo/GAZ_00002713 -->

    <owl:Class rdf:about="http://purl.obolibrary.org/obo/GAZ_00002713">
        <rdfs:subClassOf rdf:resource="http://purl.obolibrary.org/obo/GAZ_00002707"/>
    </owl:Class>
    


    <!-- http://purl.obolibrary.org/obo/GAZ_00002714 -->

    <owl:Class rdf:about="http://purl.obolibrary.org/obo/GAZ_00002714">
        <rdfs:subClassOf rdf:resource="http://purl.obolibrary.org/obo/GAZ_00002707"/>
    </owl:Class>
    


    <!-- http://purl.obolibrary.org/obo/GAZ_00003782 -->

    <owl:Class rdf:about="http://purl.obolibrary.org/obo/GAZ_00003782">
        <rdfs:subClassOf rdf:resource="http://purl.obolibrary.org/obo/GAZ_00002705"/>
    </owl:Class>
    


    <!-- http://purl.obolibrary.org/obo/GAZ_00004382 -->

    <owl:Class rdf:about="http://purl.obolibrary.org/obo/GAZ_00004382">
        <rdfs:subClassOf rdf:resource="http://purl.obolibrary.org/obo/GAZ_00002705"/>
    </owl:Class>
    


    <!-- http://purl.obolibrary.org/obo/GAZ_00004383 -->

    <owl:Class rdf:about="http://purl.obolibrary.org/obo/GAZ_00004383">
        <rdfs:subClassOf rdf:resource="http://purl.obolibrary.org/obo/GAZ_00002705"/>
    </owl:Class>
    


    <!-- http://purl.obolibrary.org/obo/GAZ_00008671 -->

    <owl:Class rdf:about="http://purl.obolibrary.org/obo/GAZ_00008671">
        <rdfs:subClassOf rdf:resource="http://purl.obolibrary.org/obo/GAZ_00002705"/>
    </owl:Class>
    


    <!-- http://purl.obolibrary.org/obo/GAZ_00010401 -->

    <owl:Class rdf:about="http://purl.obolibrary.org/obo/GAZ_00010401">
        <rdfs:subClassOf rdf:resource="http://purl.obolibrary.org/obo/GAZ_00002705"/>
    </owl:Class>
    


    <!-- http://purl.obolibrary.org/obo/GAZ_00010508 -->

    <owl:Class rdf:about="http://purl.obolibrary.org/obo/GAZ_00010508">
        <rdfs:subClassOf rdf:resource="http://purl.obolibrary.org/obo/GAZ_00002705"/>
    </owl:Class>
    


    <!-- http://purl.obolibrary.org/obo/GAZ_00010510 -->

    <owl:Class rdf:about="http://purl.obolibrary.org/obo/GAZ_00010510">
        <rdfs:subClassOf rdf:resource="http://purl.obolibrary.org/obo/GAZ_00002705"/>
    </owl:Class>
    


    <!-- http://purl.obolibrary.org/obo/GAZ_00010514 -->

    <owl:Class rdf:about="http://purl.obolibrary.org/obo/GAZ_00010514">
        <rdfs:subClassOf rdf:resource="http://purl.obolibrary.org/obo/GAZ_00002705"/>
        <oboInOwl:hasOBONamespace>GAZ</oboInOwl:hasOBONamespace>
        <oboInOwl:id>GAZ:00010514</oboInOwl:id>
        <rdfs:label>Kfar Monash</rdfs:label>
    </owl:Class>
    


    <!-- http://purl.obolibrary.org/obo/GAZ_00010516 -->

    <owl:Class rdf:about="http://purl.obolibrary.org/obo/GAZ_00010516">
        <rdfs:subClassOf rdf:resource="http://purl.obolibrary.org/obo/GAZ_00002705"/>
    </owl:Class>
    


    <!-- http://purl.obolibrary.org/obo/GAZ_00010520 -->

    <owl:Class rdf:about="http://purl.obolibrary.org/obo/GAZ_00010520">
        <rdfs:subClassOf rdf:resource="http://purl.obolibrary.org/obo/GAZ_00002705"/>
    </owl:Class>
    


    <!-- http://purl.obolibrary.org/obo/GAZ_00010525 -->

    <owl:Class rdf:about="http://purl.obolibrary.org/obo/GAZ_00010525">
        <rdfs:subClassOf rdf:resource="http://purl.obolibrary.org/obo/GAZ_00002705"/>
    </owl:Class>
    


    <!-- http://purl.obolibrary.org/obo/GAZ_00010528 -->

    <owl:Class rdf:about="http://purl.obolibrary.org/obo/GAZ_00010528">
        <rdfs:subClassOf rdf:resource="http://purl.obolibrary.org/obo/GAZ_00002705"/>
    </owl:Class>
    


    <!-- http://purl.obolibrary.org/obo/GAZ_00010529 -->

    <owl:Class rdf:about="http://purl.obolibrary.org/obo/GAZ_00010529">
        <rdfs:subClassOf rdf:resource="http://purl.obolibrary.org/obo/GAZ_00002705"/>
    </owl:Class>
    


    <!-- http://purl.obolibrary.org/obo/GAZ_00010530 -->

    <owl:Class rdf:about="http://purl.obolibrary.org/obo/GAZ_00010530">
        <rdfs:subClassOf rdf:resource="http://purl.obolibrary.org/obo/GAZ_00002705"/>
    </owl:Class>
    


    <!-- http://purl.obolibrary.org/obo/GAZ_00010531 -->

    <owl:Class rdf:about="http://purl.obolibrary.org/obo/GAZ_00010531">
        <rdfs:subClassOf rdf:resource="http://purl.obolibrary.org/obo/GAZ_00002705"/>
    </owl:Class>
    


    <!-- http://purl.obolibrary.org/obo/GAZ_00010536 -->

    <owl:Class rdf:about="http://purl.obolibrary.org/obo/GAZ_00010536">
        <rdfs:subClassOf rdf:resource="http://purl.obolibrary.org/obo/GAZ_00002705"/>
    </owl:Class>
    


    <!-- http://purl.obolibrary.org/obo/GAZ_00010537 -->

    <owl:Class rdf:about="http://purl.obolibrary.org/obo/GAZ_00010537">
        <rdfs:subClassOf rdf:resource="http://purl.obolibrary.org/obo/GAZ_00002705"/>
    </owl:Class>
    


    <!-- http://purl.obolibrary.org/obo/GAZ_00010541 -->

    <owl:Class rdf:about="http://purl.obolibrary.org/obo/GAZ_00010541">
        <rdfs:subClassOf rdf:resource="http://purl.obolibrary.org/obo/GAZ_00002705"/>
    </owl:Class>
    


    <!-- http://purl.obolibrary.org/obo/GAZ_22224108 -->

    <owl:Class rdf:about="http://purl.obolibrary.org/obo/GAZ_22224108">
        <rdfs:subClassOf rdf:resource="http://purl.obolibrary.org/obo/GAZ_00002705"/>
    </owl:Class>
    


    <!-- 
    ///////////////////////////////////////////////////////////////////////////////////////
    //
    // Individuals
    //
    ///////////////////////////////////////////////////////////////////////////////////////
     -->

    


    <!-- http://purl.obolibrary.org/obo/GAZ_00000669 -->

    <owl:NamedIndividual rdf:about="http://purl.obolibrary.org/obo/GAZ_00000669">
        <obo:IAO_0000115>One of the governorates of Egypt. It is in the east of the country, covering the northern half of the Sinai Peninsula. Its capital is Arish.</obo:IAO_0000115>
        <oboInOwl:hasOBONamespace>GAZ</oboInOwl:hasOBONamespace>
        <oboInOwl:id>GAZ:00000669</oboInOwl:id>
        <rdfs:label>North Sinai Governorate</rdfs:label>
    </owl:NamedIndividual>
    


    <!-- http://purl.obolibrary.org/obo/GAZ_00000670 -->

    <owl:NamedIndividual rdf:about="http://purl.obolibrary.org/obo/GAZ_00000670">
        <obo:IAO_0000115>One of the governorates of Egypt. It is in the east of the country, covering the southern half of the Sinai Peninsula.</obo:IAO_0000115>
        <oboInOwl:hasOBONamespace>GAZ</oboInOwl:hasOBONamespace>
        <oboInOwl:id>GAZ:00000670</oboInOwl:id>
        <rdfs:label>South Sinai Governorate</rdfs:label>
    </owl:NamedIndividual>
    


    <!-- http://purl.obolibrary.org/obo/GAZ_00002476 -->

    <owl:NamedIndividual rdf:about="http://purl.obolibrary.org/obo/GAZ_00002476">
        <rdf:type rdf:resource="http://purl.obolibrary.org/obo/ENVO_00000009"/>
        <obo:IAO_0000115>A country in Western Asia located on the eastern edge of the Mediterranean Sea. It borders Lebanon in the north, Syria in the northeast, Jordan in the east, and Egypt on the southwest. The West Bank and Gaza Strip, which are partially administrated by the Palestinian National Authority, are also adjacent. The State of Israel is divided into six main administrative districts, known as mehozot (singular mahoz). Districts are further divided into fifteen sub-districts known as nafot (singular: nafa), which are themselves partitioned into fifty natural regions.</obo:IAO_0000115>
        <oboInOwl:hasOBONamespace>GAZ</oboInOwl:hasOBONamespace>
        <oboInOwl:id>GAZ:00002476</oboInOwl:id>
        <rdfs:label>Israel</rdfs:label>
    </owl:NamedIndividual>
    


    <!-- http://purl.obolibrary.org/obo/GAZ_00002477 -->

    <owl:NamedIndividual rdf:about="http://purl.obolibrary.org/obo/GAZ_00002477">
        <obo:RO_0001025 rdf:resource="http://purl.obolibrary.org/obo/GAZ_00007520"/>
        <obo:IAO_0000115>A saline lake between the West Bank and Israel to the west, and Jordan to the east.</obo:IAO_0000115>
        <oboInOwl:hasOBONamespace>GAZ</oboInOwl:hasOBONamespace>
        <oboInOwl:id>GAZ:00002477</oboInOwl:id>
        <rdfs:label>Dead Sea</rdfs:label>
    </owl:NamedIndividual>
    


    <!-- http://purl.obolibrary.org/obo/GAZ_00002705 -->

    <owl:NamedIndividual rdf:about="http://purl.obolibrary.org/obo/GAZ_00002705">
        <obo:RO_0001025 rdf:resource="http://purl.obolibrary.org/obo/GAZ_00002476"/>
    </owl:NamedIndividual>
    


    <!-- http://purl.obolibrary.org/obo/GAZ_00002706 -->

    <owl:NamedIndividual rdf:about="http://purl.obolibrary.org/obo/GAZ_00002706">
        <obo:RO_0001025 rdf:resource="http://purl.obolibrary.org/obo/GAZ_00078261"/>
    </owl:NamedIndividual>
    


    <!-- http://purl.obolibrary.org/obo/GAZ_00002707 -->

    <owl:NamedIndividual rdf:about="http://purl.obolibrary.org/obo/GAZ_00002707">
        <obo:RO_0001025 rdf:resource="http://purl.obolibrary.org/obo/GAZ_00002476"/>
    </owl:NamedIndividual>
    


    <!-- http://purl.obolibrary.org/obo/GAZ_00002708 -->

    <owl:NamedIndividual rdf:about="http://purl.obolibrary.org/obo/GAZ_00002708"/>
    


    <!-- http://purl.obolibrary.org/obo/GAZ_00002709 -->

    <owl:NamedIndividual rdf:about="http://purl.obolibrary.org/obo/GAZ_00002709"/>
    


    <!-- http://purl.obolibrary.org/obo/GAZ_00002710 -->

    <owl:NamedIndividual rdf:about="http://purl.obolibrary.org/obo/GAZ_00002710"/>
    


    <!-- http://purl.obolibrary.org/obo/GAZ_00002711 -->

    <owl:NamedIndividual rdf:about="http://purl.obolibrary.org/obo/GAZ_00002711"/>
    


    <!-- http://purl.obolibrary.org/obo/GAZ_00002712 -->

    <owl:NamedIndividual rdf:about="http://purl.obolibrary.org/obo/GAZ_00002712"/>
    


    <!-- http://purl.obolibrary.org/obo/GAZ_00002713 -->

    <owl:NamedIndividual rdf:about="http://purl.obolibrary.org/obo/GAZ_00002713"/>
    


    <!-- http://purl.obolibrary.org/obo/GAZ_00002714 -->

    <owl:NamedIndividual rdf:about="http://purl.obolibrary.org/obo/GAZ_00002714"/>
    


    <!-- http://purl.obolibrary.org/obo/GAZ_00003782 -->

    <owl:NamedIndividual rdf:about="http://purl.obolibrary.org/obo/GAZ_00003782">
        <obo:RO_0001025 rdf:resource="http://purl.obolibrary.org/obo/GAZ_00078350"/>
    </owl:NamedIndividual>
    


    <!-- http://purl.obolibrary.org/obo/GAZ_00004382 -->

    <owl:NamedIndividual rdf:about="http://purl.obolibrary.org/obo/GAZ_00004382">
        <obo:RO_0001025 rdf:resource="http://purl.obolibrary.org/obo/GAZ_00078322"/>
    </owl:NamedIndividual>
    


    <!-- http://purl.obolibrary.org/obo/GAZ_00004383 -->

    <owl:NamedIndividual rdf:about="http://purl.obolibrary.org/obo/GAZ_00004383">
        <obo:RO_0001025 rdf:resource="http://purl.obolibrary.org/obo/GAZ_00078283"/>
    </owl:NamedIndividual>
    


    <!-- http://purl.obolibrary.org/obo/GAZ_00007520 -->

    <owl:NamedIndividual rdf:about="http://purl.obolibrary.org/obo/GAZ_00007520">
        <obo:RO_0001025 rdf:resource="http://purl.obolibrary.org/obo/GAZ_00044915"/>
        <obo:IAO_0000115>A river in Southwest Asia flowing through the Great Rift Valley into the Dead Sea.</obo:IAO_0000115>
        <oboInOwl:hasOBONamespace>GAZ</oboInOwl:hasOBONamespace>
        <oboInOwl:id>GAZ:00007520</oboInOwl:id>
        <rdfs:label>River Jordan</rdfs:label>
    </owl:NamedIndividual>
    


    <!-- http://purl.obolibrary.org/obo/GAZ_00007862 -->

    <owl:NamedIndividual rdf:about="http://purl.obolibrary.org/obo/GAZ_00007862">
        <rdf:type rdf:resource="http://purl.obolibrary.org/obo/ENVO_00000032"/>
        <obo:RO_0001025 rdf:resource="http://purl.obolibrary.org/obo/GAZ_00002710"/>
        <obo:IAO_0000115>A gulf situated northeastward and adjacent to the Red Sea, bounded by the coasts of Sinai Peninsula and Arabian Peninsula. Its southern limit with the Red Sea (in the Strait of T Degrees r Degrees n) is the following: A line joining Cape Al Qa Degrees bah (28 Degrees 01430 Seconds N - 34 Degrees 37 Minutes 15 Seconds E), in Saudi Arabia, southwestward to position 27 Degrees 58 Minutes 10 Seconds N - 34 Degrees 35 Minutes E) on the coast of T Degrees r Degrees n Island; thence from this position southward, through T Degrees r Degrees n Island, to its southwestern extremity (27 Degrees 54 Minutes 50 Seconds N - 34 Degrees 33 Minutes E); and thence from the southwestern extremity of T Degrees r Degrees n Island westward, along the parallel of 27 Degrees 54 Minutes 50 Seconds N, to the coast of Sinai Peninsula, in Egypt.</obo:IAO_0000115>
        <oboInOwl:hasOBONamespace>GAZ</oboInOwl:hasOBONamespace>
        <oboInOwl:id>GAZ:00007862</oboInOwl:id>
        <rdfs:label>Gulf of Aqaba</rdfs:label>
    </owl:NamedIndividual>
    


    <!-- http://purl.obolibrary.org/obo/GAZ_00008671 -->

    <owl:NamedIndividual rdf:about="http://purl.obolibrary.org/obo/GAZ_00008671">
        <obo:RO_0001025 rdf:resource="http://purl.obolibrary.org/obo/GAZ_00078270"/>
    </owl:NamedIndividual>
    


    <!-- http://purl.obolibrary.org/obo/GAZ_00008742 -->

    <owl:NamedIndividual rdf:about="http://purl.obolibrary.org/obo/GAZ_00008742">
        <obo:RO_0001025 rdf:resource="http://purl.obolibrary.org/obo/GAZ_00044915"/>
        <obo:IAO_0000115>A valley that lies within the northern part of the Syrian-African Rift Valley at an elevation of about 70 m above sea level. On both sides of the valley are steep slopes -- the Golan Heights to the east and the Upper Galilee mountains to the west, rise to 400 to 900 m above sea level. Basaltic hills of about 200 m above sea level along the southern side of the valley intercept the Jordan River, and are commonly referred to as the basalt &quot;plug&quot; (actually a temporary geologic base level), as they restrict water drainage downstream into the Sea of Galilee (Lake Kinneret). The Hula Valley covers an area of 177 km2 (25 km by 6-8 km.</obo:IAO_0000115>
        <oboInOwl:hasOBONamespace>GAZ</oboInOwl:hasOBONamespace>
        <oboInOwl:id>GAZ:00008742</oboInOwl:id>
        <rdfs:label>Hulah Valley</rdfs:label>
    </owl:NamedIndividual>
    


    <!-- http://purl.obolibrary.org/obo/GAZ_00008743 -->

    <owl:NamedIndividual rdf:about="http://purl.obolibrary.org/obo/GAZ_00008743">
        <obo:RO_0001025 rdf:resource="http://purl.obolibrary.org/obo/GAZ_00193886"/>
        <obo:IAO_0000115>A wetland.</obo:IAO_0000115>
        <oboInOwl:hasOBONamespace>GAZ</oboInOwl:hasOBONamespace>
        <oboInOwl:id>GAZ:00008743</oboInOwl:id>
        <rdfs:label>Hulah Swamp</rdfs:label>
    </owl:NamedIndividual>
    


    <!-- http://purl.obolibrary.org/obo/GAZ_00008823 -->

    <owl:NamedIndividual rdf:about="http://purl.obolibrary.org/obo/GAZ_00008823">
        <obo:RO_0001025 rdf:resource="http://purl.obolibrary.org/obo/GAZ_00002713"/>
        <obo:IAO_0000115>A regional council in Israel&apos;s Upper Galilee region.</obo:IAO_0000115>
        <oboInOwl:hasOBONamespace>GAZ</oboInOwl:hasOBONamespace>
        <oboInOwl:id>GAZ:00008823</oboInOwl:id>
        <rdfs:label>Upper Galilee Regional Council</rdfs:label>
    </owl:NamedIndividual>
    


    <!-- http://purl.obolibrary.org/obo/GAZ_00010400 -->

    <owl:NamedIndividual rdf:about="http://purl.obolibrary.org/obo/GAZ_00010400">
        <obo:RO_0001025 rdf:resource="http://purl.obolibrary.org/obo/GAZ_00002710"/>
        <obo:IAO_0000115>A regional council in the north-western Negev, in Israel&apos;s Southern District. The regional council&apos;s territory lies midway between Ashkelon and Beersheba, bounded on the west by the Gaza Strip while the eastern border abuts the territory of the Bnei Shimon Regional Council.</obo:IAO_0000115>
        <oboInOwl:hasOBONamespace>GAZ</oboInOwl:hasOBONamespace>
        <oboInOwl:id>GAZ:00010400</oboInOwl:id>
        <rdfs:label>Eshkol Regional Council</rdfs:label>
    </owl:NamedIndividual>
    


    <!-- http://purl.obolibrary.org/obo/GAZ_00010401 -->

    <owl:NamedIndividual rdf:about="http://purl.obolibrary.org/obo/GAZ_00010401">
        <obo:RO_0001025 rdf:resource="http://purl.obolibrary.org/obo/GAZ_00010400"/>
    </owl:NamedIndividual>
    


    <!-- http://purl.obolibrary.org/obo/GAZ_00010402 -->

    <owl:NamedIndividual rdf:about="http://purl.obolibrary.org/obo/GAZ_00010402">
        <obo:RO_0001025 rdf:resource="http://purl.obolibrary.org/obo/GAZ_00002476"/>
        <oboInOwl:hasOBONamespace>GAZ</oboInOwl:hasOBONamespace>
        <oboInOwl:id>GAZ:00010402</oboInOwl:id>
        <rdfs:label>Beit Aran</rdfs:label>
    </owl:NamedIndividual>
    


    <!-- http://purl.obolibrary.org/obo/GAZ_00010507 -->

    <owl:NamedIndividual rdf:about="http://purl.obolibrary.org/obo/GAZ_00010507">
        <obo:RO_0001025 rdf:resource="http://purl.obolibrary.org/obo/GAZ_00002710"/>
        <obo:IAO_0000115>A regional council in the southern Coastal Plain region in Israel. It borders Yoav and Nahal Sorek regional councils in the east; Hof Ashkelon regional council, the Mediterranean Sea, the city of Ashdod and Gan Yavne local council in the west; Gederot, Hevel Yavne regional councils and Gedera, Bnei Aish local councils in the north; Shafir regional council in the south. The town of Kiryat Malakhi is enclaved in the middle.</obo:IAO_0000115>
        <oboInOwl:hasOBONamespace>GAZ</oboInOwl:hasOBONamespace>
        <oboInOwl:id>GAZ:00010507</oboInOwl:id>
        <rdfs:label>Be&apos;er Tuvia Regional Council</rdfs:label>
    </owl:NamedIndividual>
    


    <!-- http://purl.obolibrary.org/obo/GAZ_00010508 -->

    <owl:NamedIndividual rdf:about="http://purl.obolibrary.org/obo/GAZ_00010508">
        <obo:RO_0001025 rdf:resource="http://purl.obolibrary.org/obo/GAZ_00010507"/>
    </owl:NamedIndividual>
    


    <!-- http://purl.obolibrary.org/obo/GAZ_00010509 -->

    <owl:NamedIndividual rdf:about="http://purl.obolibrary.org/obo/GAZ_00010509">
        <obo:RO_0001025 rdf:resource="http://purl.obolibrary.org/obo/GAZ_00002714"/>
        <obo:IAO_0000115>A populated place.</obo:IAO_0000115>
        <oboInOwl:hasOBONamespace>GAZ</oboInOwl:hasOBONamespace>
        <oboInOwl:id>GAZ:00010509</oboInOwl:id>
        <rdfs:label>Beit HaLevi</rdfs:label>
    </owl:NamedIndividual>
    


    <!-- http://purl.obolibrary.org/obo/GAZ_00010510 -->

    <owl:NamedIndividual rdf:about="http://purl.obolibrary.org/obo/GAZ_00010510">
        <obo:RO_0001025 rdf:resource="http://purl.obolibrary.org/obo/GAZ_00078282"/>
    </owl:NamedIndividual>
    


    <!-- http://purl.obolibrary.org/obo/GAZ_00010511 -->

    <owl:NamedIndividual rdf:about="http://purl.obolibrary.org/obo/GAZ_00010511">
        <obo:RO_0001025 rdf:resource="http://purl.obolibrary.org/obo/GAZ_00002476"/>
        <oboInOwl:hasOBONamespace>GAZ</oboInOwl:hasOBONamespace>
        <oboInOwl:id>GAZ:00010511</oboInOwl:id>
        <rdfs:label>Bnei Darom</rdfs:label>
    </owl:NamedIndividual>
    


    <!-- http://purl.obolibrary.org/obo/GAZ_00010512 -->

    <owl:NamedIndividual rdf:about="http://purl.obolibrary.org/obo/GAZ_00010512">
        <obo:RO_0001025 rdf:resource="http://purl.obolibrary.org/obo/GAZ_02000662"/>
        <oboInOwl:hasOBONamespace>GAZ</oboInOwl:hasOBONamespace>
        <oboInOwl:id>GAZ:00010512</oboInOwl:id>
        <rdfs:label>Sharon</rdfs:label>
    </owl:NamedIndividual>
    


    <!-- http://purl.obolibrary.org/obo/GAZ_00010513 -->

    <owl:NamedIndividual rdf:about="http://purl.obolibrary.org/obo/GAZ_00010513">
        <obo:RO_0001025 rdf:resource="http://purl.obolibrary.org/obo/GAZ_00002714"/>
        <oboInOwl:hasOBONamespace>GAZ</oboInOwl:hasOBONamespace>
        <oboInOwl:id>GAZ:00010513</oboInOwl:id>
        <rdfs:label>Pardes Hanna-Karkur</rdfs:label>
    </owl:NamedIndividual>
    


    <!-- http://purl.obolibrary.org/obo/GAZ_00010515 -->

    <owl:NamedIndividual rdf:about="http://purl.obolibrary.org/obo/GAZ_00010515">
        <obo:RO_0001025 rdf:resource="http://purl.obolibrary.org/obo/GAZ_00002476"/>
        <oboInOwl:hasOBONamespace>GAZ</oboInOwl:hasOBONamespace>
        <oboInOwl:id>GAZ:00010515</oboInOwl:id>
        <rdfs:label>Ein Habsor</rdfs:label>
    </owl:NamedIndividual>
    


    <!-- http://purl.obolibrary.org/obo/GAZ_00010516 -->

    <owl:NamedIndividual rdf:about="http://purl.obolibrary.org/obo/GAZ_00010516">
        <obo:RO_0001025 rdf:resource="http://purl.obolibrary.org/obo/GAZ_00078241"/>
    </owl:NamedIndividual>
    


    <!-- http://purl.obolibrary.org/obo/GAZ_00010519 -->

    <owl:NamedIndividual rdf:about="http://purl.obolibrary.org/obo/GAZ_00010519">
        <obo:RO_0001025 rdf:resource="http://purl.obolibrary.org/obo/GAZ_00002711"/>
        <obo:IAO_0000115>A former kibbutz located around 5 km south of Hadera in Israel. In 1952 it split into Givat Haim (Ihud) and Givat Haim (Meuhad).</obo:IAO_0000115>
        <oboInOwl:hasOBONamespace>GAZ</oboInOwl:hasOBONamespace>
        <oboInOwl:id>GAZ:00010519</oboInOwl:id>
        <rdfs:label>Givat Haim</rdfs:label>
    </owl:NamedIndividual>
    


    <!-- http://purl.obolibrary.org/obo/GAZ_00010520 -->

    <owl:NamedIndividual rdf:about="http://purl.obolibrary.org/obo/GAZ_00010520">
        <obo:RO_0001025 rdf:resource="http://purl.obolibrary.org/obo/GAZ_00078323"/>
    </owl:NamedIndividual>
    


    <!-- http://purl.obolibrary.org/obo/GAZ_00010521 -->

    <owl:NamedIndividual rdf:about="http://purl.obolibrary.org/obo/GAZ_00010521">
        <obo:RO_0001025 rdf:resource="http://purl.obolibrary.org/obo/GAZ_00010540"/>
        <obo:IAO_0000115>A moshav located north-east of Hadera (next to Pardes Hanna-Karkur), on the road to Afula, Highway 65.</obo:IAO_0000115>
        <oboInOwl:hasOBONamespace>GAZ</oboInOwl:hasOBONamespace>
        <oboInOwl:id>GAZ:00010521</oboInOwl:id>
        <rdfs:label>Gan HaShomron</rdfs:label>
    </owl:NamedIndividual>
    


    <!-- http://purl.obolibrary.org/obo/GAZ_00010522 -->

    <owl:NamedIndividual rdf:about="http://purl.obolibrary.org/obo/GAZ_00010522">
        <obo:RO_0001025 rdf:resource="http://purl.obolibrary.org/obo/GAZ_00002714"/>
        <oboInOwl:hasOBONamespace>GAZ</oboInOwl:hasOBONamespace>
        <oboInOwl:id>GAZ:00010522</oboInOwl:id>
        <rdfs:label>Kfar Vitkin</rdfs:label>
    </owl:NamedIndividual>
    


    <!-- http://purl.obolibrary.org/obo/GAZ_00010523 -->

    <owl:NamedIndividual rdf:about="http://purl.obolibrary.org/obo/GAZ_00010523">
        <obo:RO_0001025 rdf:resource="http://purl.obolibrary.org/obo/GAZ_00002714"/>
        <oboInOwl:hasOBONamespace>GAZ</oboInOwl:hasOBONamespace>
        <oboInOwl:id>GAZ:00010523</oboInOwl:id>
        <rdfs:label>Mishmar Hasharon</rdfs:label>
    </owl:NamedIndividual>
    


    <!-- http://purl.obolibrary.org/obo/GAZ_00010524 -->

    <owl:NamedIndividual rdf:about="http://purl.obolibrary.org/obo/GAZ_00010524">
        <obo:RO_0001025 rdf:resource="http://purl.obolibrary.org/obo/GAZ_00002714"/>
        <oboInOwl:hasOBONamespace>GAZ</oboInOwl:hasOBONamespace>
        <oboInOwl:id>GAZ:00010524</oboInOwl:id>
        <rdfs:label>Qevuzat Yavne</rdfs:label>
    </owl:NamedIndividual>
    


    <!-- http://purl.obolibrary.org/obo/GAZ_00010525 -->

    <owl:NamedIndividual rdf:about="http://purl.obolibrary.org/obo/GAZ_00010525">
        <rdf:type rdf:resource="http://purl.obolibrary.org/obo/ENVO_00000856"/>
        <obo:RO_0001025 rdf:resource="http://purl.obolibrary.org/obo/GAZ_00078281"/>
    </owl:NamedIndividual>
    


    <!-- http://purl.obolibrary.org/obo/GAZ_00010526 -->

    <owl:NamedIndividual rdf:about="http://purl.obolibrary.org/obo/GAZ_00010526">
        <obo:RO_0001025 rdf:resource="http://purl.obolibrary.org/obo/GAZ_00078324"/>
        <obo:IAO_0000115>A kibbutz located in the Judean hills just off the Jerusalem-Tel Aviv highway in Israel. It falls under the jurisdiction of Matte Yehuda Regional Council.</obo:IAO_0000115>
        <oboInOwl:hasOBONamespace>GAZ</oboInOwl:hasOBONamespace>
        <oboInOwl:id>GAZ:00010526</oboInOwl:id>
        <rdfs:label>Maale HaHamisha</rdfs:label>
    </owl:NamedIndividual>
    


    <!-- http://purl.obolibrary.org/obo/GAZ_00010527 -->

    <owl:NamedIndividual rdf:about="http://purl.obolibrary.org/obo/GAZ_00010527">
        <obo:RO_0001025 rdf:resource="http://purl.obolibrary.org/obo/GAZ_00078324"/>
        <obo:IAO_0000115>A moshav in central Israel. Located west of Jerusalem, it falls under the jurisdiction of Matte Yehuda Regional Council. Previously a kibbutz, it remains a member of the Kibbutz Movement despite its change in status to a moshav.</obo:IAO_0000115>
        <oboInOwl:hasOBONamespace>GAZ</oboInOwl:hasOBONamespace>
        <oboInOwl:id>GAZ:00010527</oboInOwl:id>
        <rdfs:label>Neve Ilan</rdfs:label>
    </owl:NamedIndividual>
    


    <!-- http://purl.obolibrary.org/obo/GAZ_00010528 -->

    <owl:NamedIndividual rdf:about="http://purl.obolibrary.org/obo/GAZ_00010528">
        <obo:RO_0001025 rdf:resource="http://purl.obolibrary.org/obo/GAZ_00010507"/>
    </owl:NamedIndividual>
    


    <!-- http://purl.obolibrary.org/obo/GAZ_00010529 -->

    <owl:NamedIndividual rdf:about="http://purl.obolibrary.org/obo/GAZ_00010529">
        <obo:RO_0001025 rdf:resource="http://purl.obolibrary.org/obo/GAZ_00010540"/>
    </owl:NamedIndividual>
    


    <!-- http://purl.obolibrary.org/obo/GAZ_00010530 -->

    <owl:NamedIndividual rdf:about="http://purl.obolibrary.org/obo/GAZ_00010530">
        <rdf:type rdf:resource="http://purl.obolibrary.org/obo/ENVO_00000062"/>
        <obo:RO_0001025 rdf:resource="http://purl.obolibrary.org/obo/GAZ_00010534"/>
    </owl:NamedIndividual>
    


    <!-- http://purl.obolibrary.org/obo/GAZ_00010531 -->

    <owl:NamedIndividual rdf:about="http://purl.obolibrary.org/obo/GAZ_00010531">
        <obo:RO_0001025 rdf:resource="http://purl.obolibrary.org/obo/GAZ_00010534"/>
    </owl:NamedIndividual>
    


    <!-- http://purl.obolibrary.org/obo/GAZ_00010532 -->

    <owl:NamedIndividual rdf:about="http://purl.obolibrary.org/obo/GAZ_00010532">
        <obo:RO_0001025 rdf:resource="http://purl.obolibrary.org/obo/GAZ_00002713"/>
        <obo:IAO_0000115>A regional council in northern Israel that encompasses most of the settlements in the Lower Galilee.</obo:IAO_0000115>
        <oboInOwl:hasOBONamespace>GAZ</oboInOwl:hasOBONamespace>
        <oboInOwl:id>GAZ:00010532</oboInOwl:id>
        <rdfs:label>Lower Galilee Regional Council</rdfs:label>
    </owl:NamedIndividual>
    


    <!-- http://purl.obolibrary.org/obo/GAZ_00010533 -->

    <owl:NamedIndividual rdf:about="http://purl.obolibrary.org/obo/GAZ_00010533">
        <obo:RO_0001025 rdf:resource="http://purl.obolibrary.org/obo/GAZ_00044915"/>
        <obo:IAO_0000115>A large fertile plain and inland valley in the south of the Lower Galilee region of Israel. It is bordered to the south by the Samaria highlands and Mount Gilboa, to the north by the Lower Galilee, to the west by the Mount Carmel range, and to the east by the Jordan Valley.</obo:IAO_0000115>
        <oboInOwl:hasOBONamespace>GAZ</oboInOwl:hasOBONamespace>
        <oboInOwl:id>GAZ:00010533</oboInOwl:id>
        <rdfs:label>Jezreel Valley</rdfs:label>
    </owl:NamedIndividual>
    


    <!-- http://purl.obolibrary.org/obo/GAZ_00010534 -->

    <owl:NamedIndividual rdf:about="http://purl.obolibrary.org/obo/GAZ_00010534">
        <obo:RO_0001025 rdf:resource="http://purl.obolibrary.org/obo/GAZ_00002713"/>
        <obo:IAO_0000115>A regional council in northern Israel that encompasses most of the settlements in the Jezreel Valley. It includes 15 kibbutzim, 15 moshavim, 6 Jewish villages, and 2 minority villages. Despite its name, some of these settlements are not located in the Jezreel Valley proper, but in the vicinity.</obo:IAO_0000115>
        <oboInOwl:hasOBONamespace>GAZ</oboInOwl:hasOBONamespace>
        <oboInOwl:id>GAZ:00010534</oboInOwl:id>
        <rdfs:label>Jezreel Valley Regional Council</rdfs:label>
    </owl:NamedIndividual>
    


    <!-- http://purl.obolibrary.org/obo/GAZ_00010535 -->

    <owl:NamedIndividual rdf:about="http://purl.obolibrary.org/obo/GAZ_00010535">
        <obo:RO_0001025 rdf:resource="http://purl.obolibrary.org/obo/GAZ_00078361"/>
        <obo:IAO_0000115>A kibbutz in the Northern District of Israel, near the Gilboa ridge.</obo:IAO_0000115>
        <oboInOwl:hasOBONamespace>GAZ</oboInOwl:hasOBONamespace>
        <oboInOwl:id>GAZ:00010535</oboInOwl:id>
        <rdfs:label>Beit Alfa</rdfs:label>
    </owl:NamedIndividual>
    


    <!-- http://purl.obolibrary.org/obo/GAZ_00010536 -->

    <owl:NamedIndividual rdf:about="http://purl.obolibrary.org/obo/GAZ_00010536">
        <obo:RO_0001025 rdf:resource="http://purl.obolibrary.org/obo/GAZ_00002713"/>
    </owl:NamedIndividual>
    


    <!-- http://purl.obolibrary.org/obo/GAZ_00010537 -->

    <owl:NamedIndividual rdf:about="http://purl.obolibrary.org/obo/GAZ_00010537">
        <obo:RO_0001025 rdf:resource="http://purl.obolibrary.org/obo/GAZ_00010507"/>
    </owl:NamedIndividual>
    


    <!-- http://purl.obolibrary.org/obo/GAZ_00010538 -->

    <owl:NamedIndividual rdf:about="http://purl.obolibrary.org/obo/GAZ_00010538">
        <obo:RO_0001025 rdf:resource="http://purl.obolibrary.org/obo/GAZ_00002476"/>
        <oboInOwl:hasOBONamespace>GAZ</oboInOwl:hasOBONamespace>
        <oboInOwl:id>GAZ:00010538</oboInOwl:id>
        <rdfs:label>Tzur Moshe</rdfs:label>
    </owl:NamedIndividual>
    


    <!-- http://purl.obolibrary.org/obo/GAZ_00010539 -->

    <owl:NamedIndividual rdf:about="http://purl.obolibrary.org/obo/GAZ_00010539">
        <rdf:type rdf:resource="http://purl.obolibrary.org/obo/ENVO_00000062"/>
        <obo:RO_0001025 rdf:resource="http://purl.obolibrary.org/obo/GAZ_00002714"/>
        <obo:IAO_0000115>A place in Center District, Israel.</obo:IAO_0000115>
        <oboInOwl:hasOBONamespace>GAZ</oboInOwl:hasOBONamespace>
        <oboInOwl:id>GAZ:00010539</oboInOwl:id>
        <rdfs:label>Yesodot</rdfs:label>
    </owl:NamedIndividual>
    


    <!-- http://purl.obolibrary.org/obo/GAZ_00010540 -->

    <owl:NamedIndividual rdf:about="http://purl.obolibrary.org/obo/GAZ_00010540">
        <obo:RO_0001025 rdf:resource="http://purl.obolibrary.org/obo/GAZ_00002711"/>
        <obo:IAO_0000115>A regional council near the city of Hadera, on Israel&apos;s north-central coastal plain in the southern Haifa District.</obo:IAO_0000115>
        <oboInOwl:hasOBONamespace>GAZ</oboInOwl:hasOBONamespace>
        <oboInOwl:id>GAZ:00010540</oboInOwl:id>
        <rdfs:label>Menashe Regional Council</rdfs:label>
    </owl:NamedIndividual>
    


    <!-- http://purl.obolibrary.org/obo/GAZ_00010541 -->

    <owl:NamedIndividual rdf:about="http://purl.obolibrary.org/obo/GAZ_00010541">
        <obo:RO_0001025 rdf:resource="http://purl.obolibrary.org/obo/GAZ_00010540"/>
    </owl:NamedIndividual>
    


    <!-- http://purl.obolibrary.org/obo/GAZ_00010542 -->

    <owl:NamedIndividual rdf:about="http://purl.obolibrary.org/obo/GAZ_00010542">
        <obo:RO_0001025 rdf:resource="http://purl.obolibrary.org/obo/GAZ_00078271"/>
        <obo:IAO_0000115>An ancient port city located south of Tel Aviv, Israel on the Mediterranean Sea. Today it is a borough of the city.</obo:IAO_0000115>
        <oboInOwl:hasOBONamespace>GAZ</oboInOwl:hasOBONamespace>
        <oboInOwl:id>GAZ:00010542</oboInOwl:id>
        <rdfs:label>Jaffa</rdfs:label>
    </owl:NamedIndividual>
    


    <!-- http://purl.obolibrary.org/obo/GAZ_00030972 -->

    <owl:NamedIndividual rdf:about="http://purl.obolibrary.org/obo/GAZ_00030972">
        <obo:RO_0001025 rdf:resource="http://purl.obolibrary.org/obo/GAZ_00000670"/>
        <obo:IAO_0000115>An administrative region (kism) of South Sinai Governorate.</obo:IAO_0000115>
        <oboInOwl:hasOBONamespace>GAZ</oboInOwl:hasOBONamespace>
        <oboInOwl:id>GAZ:00030972</oboInOwl:id>
        <rdfs:label>Kism Abu Zanimah</rdfs:label>
    </owl:NamedIndividual>
    


    <!-- http://purl.obolibrary.org/obo/GAZ_00030973 -->

    <owl:NamedIndividual rdf:about="http://purl.obolibrary.org/obo/GAZ_00030973">
        <obo:RO_0001025 rdf:resource="http://purl.obolibrary.org/obo/GAZ_00000670"/>
        <obo:IAO_0000115>An administrative region (kism) of South Sinai Governorate.</obo:IAO_0000115>
        <oboInOwl:hasOBONamespace>GAZ</oboInOwl:hasOBONamespace>
        <oboInOwl:id>GAZ:00030973</oboInOwl:id>
        <rdfs:label>Kism At Tur</rdfs:label>
    </owl:NamedIndividual>
    


    <!-- http://purl.obolibrary.org/obo/GAZ_00030974 -->

    <owl:NamedIndividual rdf:about="http://purl.obolibrary.org/obo/GAZ_00030974">
        <obo:RO_0001025 rdf:resource="http://purl.obolibrary.org/obo/GAZ_00000670"/>
        <obo:IAO_0000115>An administrative region (kism) of South Sinai Governorate.</obo:IAO_0000115>
        <oboInOwl:hasOBONamespace>GAZ</oboInOwl:hasOBONamespace>
        <oboInOwl:id>GAZ:00030974</oboInOwl:id>
        <rdfs:label>Kism Ras Sudr</rdfs:label>
    </owl:NamedIndividual>
    


    <!-- http://purl.obolibrary.org/obo/GAZ_00030975 -->

    <owl:NamedIndividual rdf:about="http://purl.obolibrary.org/obo/GAZ_00030975">
        <obo:RO_0001025 rdf:resource="http://purl.obolibrary.org/obo/GAZ_00000670"/>
        <obo:IAO_0000115>An administrative region (kism) of South Sinai Governorate.</obo:IAO_0000115>
        <oboInOwl:hasOBONamespace>GAZ</oboInOwl:hasOBONamespace>
        <oboInOwl:id>GAZ:00030975</oboInOwl:id>
        <rdfs:label>Kism Al Qiddisah Katrina</rdfs:label>
    </owl:NamedIndividual>
    


    <!-- http://purl.obolibrary.org/obo/GAZ_00030976 -->

    <owl:NamedIndividual rdf:about="http://purl.obolibrary.org/obo/GAZ_00030976">
        <obo:RO_0001025 rdf:resource="http://purl.obolibrary.org/obo/GAZ_00000670"/>
        <obo:IAO_0000115>An administrative region (kism) of South Sinai Governorate.</obo:IAO_0000115>
        <oboInOwl:hasOBONamespace>GAZ</oboInOwl:hasOBONamespace>
        <oboInOwl:id>GAZ:00030976</oboInOwl:id>
        <rdfs:label>Kism Sharm ash Shaykh</rdfs:label>
    </owl:NamedIndividual>
    


    <!-- http://purl.obolibrary.org/obo/GAZ_00030977 -->

    <owl:NamedIndividual rdf:about="http://purl.obolibrary.org/obo/GAZ_00030977">
        <obo:RO_0001025 rdf:resource="http://purl.obolibrary.org/obo/GAZ_00000670"/>
        <obo:IAO_0000115>An administrative region (kism) of South Sinai Governorate.</obo:IAO_0000115>
        <oboInOwl:hasOBONamespace>GAZ</oboInOwl:hasOBONamespace>
        <oboInOwl:id>GAZ:00030977</oboInOwl:id>
        <rdfs:label>Kism Abu Rudays</rdfs:label>
    </owl:NamedIndividual>
    


    <!-- http://purl.obolibrary.org/obo/GAZ_00030979 -->

    <owl:NamedIndividual rdf:about="http://purl.obolibrary.org/obo/GAZ_00030979">
        <obo:RO_0001025 rdf:resource="http://purl.obolibrary.org/obo/GAZ_00000670"/>
        <obo:IAO_0000115>An administrative region of South Sinai Governorate.</obo:IAO_0000115>
        <oboInOwl:hasOBONamespace>GAZ</oboInOwl:hasOBONamespace>
        <oboInOwl:id>GAZ:00030979</oboInOwl:id>
        <rdfs:label>Taba Region</rdfs:label>
    </owl:NamedIndividual>
    


    <!-- http://purl.obolibrary.org/obo/GAZ_00030980 -->

    <owl:NamedIndividual rdf:about="http://purl.obolibrary.org/obo/GAZ_00030980">
        <obo:RO_0001025 rdf:resource="http://purl.obolibrary.org/obo/GAZ_00000670"/>
        <obo:IAO_0000115>An administrative region (kism) of South Sinai Governorate.</obo:IAO_0000115>
        <oboInOwl:hasOBONamespace>GAZ</oboInOwl:hasOBONamespace>
        <oboInOwl:id>GAZ:00030980</oboInOwl:id>
        <rdfs:label>Kism Nuwaybi&apos;a</rdfs:label>
    </owl:NamedIndividual>
    


    <!-- http://purl.obolibrary.org/obo/GAZ_00044914 -->

    <owl:NamedIndividual rdf:about="http://purl.obolibrary.org/obo/GAZ_00044914">
        <obo:RO_0001025 rdf:resource="http://purl.obolibrary.org/obo/GAZ_00002476"/>
        <obo:RO_0001025 rdf:resource="http://purl.obolibrary.org/obo/GAZ_00007520"/>
        <obo:IAO_0000115>A freshwater monomictic lake, being approximately 53 km in circumference, about 21 km long, and 13 km wide. The lake has a total area of 166 km2, and a maximum depth of approximately 43 m. It is situated deep in the Jordan Great Rift Valley, the valley caused by the separation of the African and Arabian Plates and is fed partly by underground springs although its main source is the Jordan River which flows through it from north to south. Consequently the area is subject to earthquakes and, in the past, volcanic activity. This is evidenced by the abundant basalt and other igneous rocks that define the geology of the Galilee region.</obo:IAO_0000115>
        <oboInOwl:hasOBONamespace>GAZ</oboInOwl:hasOBONamespace>
        <oboInOwl:id>GAZ:00044914</oboInOwl:id>
        <rdfs:label>Sea of Galilee</rdfs:label>
    </owl:NamedIndividual>
    


    <!-- http://purl.obolibrary.org/obo/GAZ_00044915 -->

    <owl:NamedIndividual rdf:about="http://purl.obolibrary.org/obo/GAZ_00044915">
        <obo:IAO_0000115>A 375 km long strike-slip fault zone some 5 km wide in the north and 23 km wide in the south that forms part of the broader Great Rift Valley. Located in modern-day Israel, Jordan, the West Bank and the Golan Heights, this geographic region includes the Jordan River, Hula Valley, Lake Tiberias and the Dead Sea, features created by the physiographic and geologic process underway.</obo:IAO_0000115>
        <oboInOwl:hasOBONamespace>GAZ</oboInOwl:hasOBONamespace>
        <oboInOwl:id>GAZ:00044915</oboInOwl:id>
        <rdfs:label>Jordan Rift Valley</rdfs:label>
    </owl:NamedIndividual>
    


    <!-- http://purl.obolibrary.org/obo/GAZ_00044916 -->

    <owl:NamedIndividual rdf:about="http://purl.obolibrary.org/obo/GAZ_00044916">
        <obo:RO_0001025 rdf:resource="http://purl.obolibrary.org/obo/GAZ_00044915"/>
        <obo:IAO_0000115>A section of the Great Rift Valley lying between the Dead Sea to the north and the Gulf of Aqaba or the Gulf of Eilat to the south. It forms part of the border between Israel to the west and Jordan to the east.</obo:IAO_0000115>
        <oboInOwl:hasOBONamespace>GAZ</oboInOwl:hasOBONamespace>
        <oboInOwl:id>GAZ:00044916</oboInOwl:id>
        <rdfs:label>Wadi Arabah</rdfs:label>
    </owl:NamedIndividual>
    


    <!-- http://purl.obolibrary.org/obo/GAZ_00049007 -->

    <owl:NamedIndividual rdf:about="http://purl.obolibrary.org/obo/GAZ_00049007">
        <obo:RO_0001025 rdf:resource="http://purl.obolibrary.org/obo/GAZ_00007862"/>
        <obo:IAO_0000115>The narrow sea passages, about 13 km wide, between the Sinai and Arabian peninsulas which separates the Gulf of Aqaba from the Red Sea.</obo:IAO_0000115>
        <oboInOwl:hasOBONamespace>GAZ</oboInOwl:hasOBONamespace>
        <oboInOwl:id>GAZ:00049007</oboInOwl:id>
        <rdfs:label>Straits of Tiran</rdfs:label>
    </owl:NamedIndividual>
    


    <!-- http://purl.obolibrary.org/obo/GAZ_00049008 -->

    <owl:NamedIndividual rdf:about="http://purl.obolibrary.org/obo/GAZ_00049008">
        <obo:RO_0001025 rdf:resource="http://purl.obolibrary.org/obo/GAZ_00049007"/>
        <obo:RO_0001025 rdf:resource="http://purl.obolibrary.org/obo/GAZ_00089762"/>
        <obo:IAO_0000115>A Saudi Arabian island in the Straits of Tiran east of Tiran Island.</obo:IAO_0000115>
        <oboInOwl:hasOBONamespace>GAZ</oboInOwl:hasOBONamespace>
        <oboInOwl:id>GAZ:00049008</oboInOwl:id>
        <rdfs:label>Sanafir Island</rdfs:label>
    </owl:NamedIndividual>
    


    <!-- http://purl.obolibrary.org/obo/GAZ_00049009 -->

    <owl:NamedIndividual rdf:about="http://purl.obolibrary.org/obo/GAZ_00049009">
        <obo:RO_0001025 rdf:resource="http://purl.obolibrary.org/obo/GAZ_00049007"/>
        <obo:RO_0001025 rdf:resource="http://purl.obolibrary.org/obo/GAZ_00089762"/>
        <obo:IAO_0000115>An island belonging to Saudi Arabia at the entrance of the Straits of Tiran, which separates the Red Sea and the Gulf of Aqaba.</obo:IAO_0000115>
        <oboInOwl:hasOBONamespace>GAZ</oboInOwl:hasOBONamespace>
        <oboInOwl:id>GAZ:00049009</oboInOwl:id>
        <rdfs:label>Tiran Island</rdfs:label>
    </owl:NamedIndividual>
    


    <!-- http://purl.obolibrary.org/obo/GAZ_00052883 -->

    <owl:NamedIndividual rdf:about="http://purl.obolibrary.org/obo/GAZ_00052883">
        <obo:IAO_0000115>A dam on the Yarmuk River.</obo:IAO_0000115>
        <oboInOwl:hasOBONamespace>GAZ</oboInOwl:hasOBONamespace>
        <oboInOwl:id>GAZ:00052883</oboInOwl:id>
        <rdfs:label>Maqarin Dam</rdfs:label>
    </owl:NamedIndividual>
    


    <!-- http://purl.obolibrary.org/obo/GAZ_00053683 -->

    <owl:NamedIndividual rdf:about="http://purl.obolibrary.org/obo/GAZ_00053683">
        <obo:IAO_0000115>A volcanic field in the Anti-Lebanon Mountains of SW Syria near the borders with Lebanon and Israel contains numerous cinder cones of Pliocene-to-Holocene age. The Golan Heights volcanic field covers a broad area NE of the Lake Tiberius (the Sea of Galilee) and SW of the city of Damascus (Dimashq) and includes the prehistoric cone of Majdel Shams in the Golan Heights. The volcanic field lies on a basaltic plateau that dips to the west and SW, with steep slopes facing the Dead Sea rift valley. It lies within the northern part of the massive alkaline Harrat Ash Shaam volcanic field that extends from southern Syria through NW Jordan to Saudi Arabia.</obo:IAO_0000115>
        <oboInOwl:hasOBONamespace>GAZ</oboInOwl:hasOBONamespace>
        <oboInOwl:id>GAZ:00053683</oboInOwl:id>
        <rdfs:label>Golan Heights Volcanic Field</rdfs:label>
    </owl:NamedIndividual>
    


    <!-- http://purl.obolibrary.org/obo/GAZ_00057703 -->

    <owl:NamedIndividual rdf:about="http://purl.obolibrary.org/obo/GAZ_00057703">
        <obo:RO_0001025 rdf:resource="http://purl.obolibrary.org/obo/GAZ_00002476"/>
        <obo:IAO_0000115>A desert located east of Jerusalem, which descends in a series of steps to the Dead Sea.</obo:IAO_0000115>
        <oboInOwl:hasOBONamespace>GAZ</oboInOwl:hasOBONamespace>
        <oboInOwl:id>GAZ:00057703</oboInOwl:id>
        <rdfs:label>Judean Desert</rdfs:label>
    </owl:NamedIndividual>
    


    <!-- http://purl.obolibrary.org/obo/GAZ_00057704 -->

    <owl:NamedIndividual rdf:about="http://purl.obolibrary.org/obo/GAZ_00057704">
        <obo:RO_0001025 rdf:resource="http://purl.obolibrary.org/obo/GAZ_00002476"/>
        <obo:RO_0001025 rdf:resource="http://purl.obolibrary.org/obo/GAZ_00002710"/>
        <obo:IAO_0000115>A desert that forms a triangle shape whose western side is contiguous with the desert of the Sinai Peninsula, and whose eastern border is the Wadi Arabah.</obo:IAO_0000115>
        <oboInOwl:hasOBONamespace>GAZ</oboInOwl:hasOBONamespace>
        <oboInOwl:id>GAZ:00057704</oboInOwl:id>
        <rdfs:label>Negev Desert</rdfs:label>
    </owl:NamedIndividual>
    


    <!-- http://purl.obolibrary.org/obo/GAZ_00058383 -->

    <owl:NamedIndividual rdf:about="http://purl.obolibrary.org/obo/GAZ_00058383">
        <obo:RO_0001025 rdf:resource="http://purl.obolibrary.org/obo/GAZ_00053683"/>
        <obo:IAO_0000115>A crater lake in the northeastern Golan Heights, near Mount Hermon.</obo:IAO_0000115>
        <oboInOwl:hasOBONamespace>GAZ</oboInOwl:hasOBONamespace>
        <oboInOwl:id>GAZ:00058383</oboInOwl:id>
        <rdfs:label>Birkat Ram</rdfs:label>
    </owl:NamedIndividual>
    


    <!-- http://purl.obolibrary.org/obo/GAZ_00058384 -->

    <owl:NamedIndividual rdf:about="http://purl.obolibrary.org/obo/GAZ_00058384">
        <obo:RO_0001025 rdf:resource="http://purl.obolibrary.org/obo/GAZ_00008742"/>
        <obo:IAO_0000115>A lake that was drained in the 1950s, but is now being regenerated.</obo:IAO_0000115>
        <oboInOwl:hasOBONamespace>GAZ</oboInOwl:hasOBONamespace>
        <oboInOwl:id>GAZ:00058384</oboInOwl:id>
        <rdfs:label>Lake Hulah</rdfs:label>
    </owl:NamedIndividual>
    


    <!-- http://purl.obolibrary.org/obo/GAZ_00058991 -->

    <owl:NamedIndividual rdf:about="http://purl.obolibrary.org/obo/GAZ_00058991">
        <obo:RO_0001025 rdf:resource="http://purl.obolibrary.org/obo/GAZ_00002476"/>
        <obo:IAO_0000115>A reservoir in Israel.</obo:IAO_0000115>
        <oboInOwl:hasOBONamespace>GAZ</oboInOwl:hasOBONamespace>
        <oboInOwl:id>GAZ:00058991</oboInOwl:id>
        <rdfs:label>Kishon Reservoir</rdfs:label>
    </owl:NamedIndividual>
    


    <!-- http://purl.obolibrary.org/obo/GAZ_00066418 -->

    <owl:NamedIndividual rdf:about="http://purl.obolibrary.org/obo/GAZ_00066418">
        <obo:RO_0001025 rdf:resource="http://purl.obolibrary.org/obo/GAZ_00000669"/>
        <obo:IAO_0000115>An administrative region (markaz) of North Sinai Governorate.</obo:IAO_0000115>
        <oboInOwl:hasOBONamespace>GAZ</oboInOwl:hasOBONamespace>
        <oboInOwl:id>GAZ:00066418</oboInOwl:id>
        <rdfs:label>Alsheikh Zwayed Region</rdfs:label>
    </owl:NamedIndividual>
    


    <!-- http://purl.obolibrary.org/obo/GAZ_00066423 -->

    <owl:NamedIndividual rdf:about="http://purl.obolibrary.org/obo/GAZ_00066423">
        <obo:RO_0001025 rdf:resource="http://purl.obolibrary.org/obo/GAZ_00000669"/>
        <oboInOwl:hasOBONamespace>GAZ</oboInOwl:hasOBONamespace>
        <oboInOwl:id>GAZ:00066423</oboInOwl:id>
        <rdfs:label>Alaresh Region</rdfs:label>
    </owl:NamedIndividual>
    


    <!-- http://purl.obolibrary.org/obo/GAZ_00066424 -->

    <owl:NamedIndividual rdf:about="http://purl.obolibrary.org/obo/GAZ_00066424">
        <obo:RO_0001025 rdf:resource="http://purl.obolibrary.org/obo/GAZ_00000669"/>
        <obo:IAO_0000115>An administrative region (markaz) of North Sinai Governorate.</obo:IAO_0000115>
        <oboInOwl:hasOBONamespace>GAZ</oboInOwl:hasOBONamespace>
        <oboInOwl:id>GAZ:00066424</oboInOwl:id>
        <rdfs:label>Nekhel Region</rdfs:label>
    </owl:NamedIndividual>
    


    <!-- http://purl.obolibrary.org/obo/GAZ_00066425 -->

    <owl:NamedIndividual rdf:about="http://purl.obolibrary.org/obo/GAZ_00066425">
        <obo:RO_0001025 rdf:resource="http://purl.obolibrary.org/obo/GAZ_00000669"/>
        <obo:IAO_0000115>An administrative region (markaz) of North Sinai Governorate.</obo:IAO_0000115>
        <oboInOwl:hasOBONamespace>GAZ</oboInOwl:hasOBONamespace>
        <oboInOwl:id>GAZ:00066425</oboInOwl:id>
        <rdfs:label>Alhasanah Region</rdfs:label>
    </owl:NamedIndividual>
    


    <!-- http://purl.obolibrary.org/obo/GAZ_00066426 -->

    <owl:NamedIndividual rdf:about="http://purl.obolibrary.org/obo/GAZ_00066426">
        <obo:RO_0001025 rdf:resource="http://purl.obolibrary.org/obo/GAZ_00000669"/>
        <obo:IAO_0000115>An administrative region (markaz) of North Sinai Governorate.</obo:IAO_0000115>
        <oboInOwl:hasOBONamespace>GAZ</oboInOwl:hasOBONamespace>
        <oboInOwl:id>GAZ:00066426</oboInOwl:id>
        <rdfs:label>Rafah Region</rdfs:label>
    </owl:NamedIndividual>
    


    <!-- http://purl.obolibrary.org/obo/GAZ_00066427 -->

    <owl:NamedIndividual rdf:about="http://purl.obolibrary.org/obo/GAZ_00066427">
        <obo:RO_0001025 rdf:resource="http://purl.obolibrary.org/obo/GAZ_00000669"/>
        <obo:IAO_0000115>An administrative region (kism) of North Sinai Governorate.</obo:IAO_0000115>
        <oboInOwl:hasOBONamespace>GAZ</oboInOwl:hasOBONamespace>
        <oboInOwl:id>GAZ:00066427</oboInOwl:id>
        <rdfs:label>Kism Bi&apos;r al&apos;Abd</rdfs:label>
    </owl:NamedIndividual>
    


    <!-- http://purl.obolibrary.org/obo/GAZ_00076360 -->

    <owl:NamedIndividual rdf:about="http://purl.obolibrary.org/obo/GAZ_00076360">
        <obo:RO_0001025 rdf:resource="http://purl.obolibrary.org/obo/GAZ_00000670"/>
        <obo:IAO_0000115>A national park. Established 1988.</obo:IAO_0000115>
        <oboInOwl:hasOBONamespace>GAZ</oboInOwl:hasOBONamespace>
        <oboInOwl:id>GAZ:00076360</oboInOwl:id>
        <rdfs:label>Saint Catherine National Park</rdfs:label>
    </owl:NamedIndividual>
    


    <!-- http://purl.obolibrary.org/obo/GAZ_00078176 -->

    <owl:NamedIndividual rdf:about="http://purl.obolibrary.org/obo/GAZ_00078176">
        <obo:RO_0001025 rdf:resource="http://purl.obolibrary.org/obo/GAZ_00002708"/>
        <oboInOwl:hasOBONamespace>GAZ</oboInOwl:hasOBONamespace>
        <oboInOwl:id>GAZ:00078176</oboInOwl:id>
        <rdfs:label>Jerusalem Subdistrict</rdfs:label>
    </owl:NamedIndividual>
    


    <!-- http://purl.obolibrary.org/obo/GAZ_00078177 -->

    <owl:NamedIndividual rdf:about="http://purl.obolibrary.org/obo/GAZ_00078177">
        <obo:RO_0001025 rdf:resource="http://purl.obolibrary.org/obo/GAZ_00078176"/>
        <oboInOwl:hasOBONamespace>GAZ</oboInOwl:hasOBONamespace>
        <oboInOwl:id>GAZ:00078177</oboInOwl:id>
        <rdfs:label>Judean Footthills Region</rdfs:label>
    </owl:NamedIndividual>
    


    <!-- http://purl.obolibrary.org/obo/GAZ_00078178 -->

    <owl:NamedIndividual rdf:about="http://purl.obolibrary.org/obo/GAZ_00078178">
        <obo:RO_0001025 rdf:resource="http://purl.obolibrary.org/obo/GAZ_00078176"/>
        <oboInOwl:hasOBONamespace>GAZ</oboInOwl:hasOBONamespace>
        <oboInOwl:id>GAZ:00078178</oboInOwl:id>
        <rdfs:label>Judean Mountains Region</rdfs:label>
    </owl:NamedIndividual>
    


    <!-- http://purl.obolibrary.org/obo/GAZ_00078179 -->

    <owl:NamedIndividual rdf:about="http://purl.obolibrary.org/obo/GAZ_00078179">
        <obo:RO_0001025 rdf:resource="http://purl.obolibrary.org/obo/GAZ_02000665"/>
        <oboInOwl:hasOBONamespace>GAZ</oboInOwl:hasOBONamespace>
        <oboInOwl:id>GAZ:00078179</oboInOwl:id>
        <rdfs:label>Hazor Region</rdfs:label>
    </owl:NamedIndividual>
    


    <!-- http://purl.obolibrary.org/obo/GAZ_00078180 -->

    <owl:NamedIndividual rdf:about="http://purl.obolibrary.org/obo/GAZ_00078180">
        <obo:RO_0001025 rdf:resource="http://purl.obolibrary.org/obo/GAZ_02000665"/>
        <oboInOwl:hasOBONamespace>GAZ</oboInOwl:hasOBONamespace>
        <oboInOwl:id>GAZ:00078180</oboInOwl:id>
        <rdfs:label>Eastern Upper Galilee Region</rdfs:label>
    </owl:NamedIndividual>
    


    <!-- http://purl.obolibrary.org/obo/GAZ_00078181 -->

    <owl:NamedIndividual rdf:about="http://purl.obolibrary.org/obo/GAZ_00078181">
        <obo:RO_0001025 rdf:resource="http://purl.obolibrary.org/obo/GAZ_02000665"/>
        <oboInOwl:hasOBONamespace>GAZ</oboInOwl:hasOBONamespace>
        <oboInOwl:id>GAZ:00078181</oboInOwl:id>
        <rdfs:label>Hula Basin Region</rdfs:label>
    </owl:NamedIndividual>
    


    <!-- http://purl.obolibrary.org/obo/GAZ_00078182 -->

    <owl:NamedIndividual rdf:about="http://purl.obolibrary.org/obo/GAZ_00078182">
        <obo:RO_0001025 rdf:resource="http://purl.obolibrary.org/obo/GAZ_02000663"/>
        <oboInOwl:hasOBONamespace>GAZ</oboInOwl:hasOBONamespace>
        <oboInOwl:id>GAZ:00078182</oboInOwl:id>
        <rdfs:label>Eastern Lower Galilee Region</rdfs:label>
    </owl:NamedIndividual>
    


    <!-- http://purl.obolibrary.org/obo/GAZ_00078183 -->

    <owl:NamedIndividual rdf:about="http://purl.obolibrary.org/obo/GAZ_00078183">
        <obo:RO_0001025 rdf:resource="http://purl.obolibrary.org/obo/GAZ_02000663"/>
        <oboInOwl:hasOBONamespace>GAZ</oboInOwl:hasOBONamespace>
        <oboInOwl:id>GAZ:00078183</oboInOwl:id>
        <rdfs:label>Kinerot Region</rdfs:label>
    </owl:NamedIndividual>
    


    <!-- http://purl.obolibrary.org/obo/GAZ_00078184 -->

    <owl:NamedIndividual rdf:about="http://purl.obolibrary.org/obo/GAZ_00078184">
        <obo:RO_0001025 rdf:resource="http://purl.obolibrary.org/obo/GAZ_02000667"/>
        <oboInOwl:hasOBONamespace>GAZ</oboInOwl:hasOBONamespace>
        <oboInOwl:id>GAZ:00078184</oboInOwl:id>
        <rdfs:label>Yoqne&apos;am Region</rdfs:label>
    </owl:NamedIndividual>
    


    <!-- http://purl.obolibrary.org/obo/GAZ_00078185 -->

    <owl:NamedIndividual rdf:about="http://purl.obolibrary.org/obo/GAZ_00078185">
        <obo:RO_0001025 rdf:resource="http://purl.obolibrary.org/obo/GAZ_02000667"/>
        <oboInOwl:hasOBONamespace>GAZ</oboInOwl:hasOBONamespace>
        <oboInOwl:id>GAZ:00078185</oboInOwl:id>
        <rdfs:label>Menashe Plateau Region</rdfs:label>
    </owl:NamedIndividual>
    


    <!-- http://purl.obolibrary.org/obo/GAZ_00078186 -->

    <owl:NamedIndividual rdf:about="http://purl.obolibrary.org/obo/GAZ_00078186">
        <obo:RO_0001025 rdf:resource="http://purl.obolibrary.org/obo/GAZ_02000667"/>
        <oboInOwl:hasOBONamespace>GAZ</oboInOwl:hasOBONamespace>
        <oboInOwl:id>GAZ:00078186</oboInOwl:id>
        <rdfs:label>Bet She&apos;an Basin Region</rdfs:label>
    </owl:NamedIndividual>
    


    <!-- http://purl.obolibrary.org/obo/GAZ_00078187 -->

    <owl:NamedIndividual rdf:about="http://purl.obolibrary.org/obo/GAZ_00078187">
        <obo:RO_0001025 rdf:resource="http://purl.obolibrary.org/obo/GAZ_02000667"/>
        <oboInOwl:hasOBONamespace>GAZ</oboInOwl:hasOBONamespace>
        <oboInOwl:id>GAZ:00078187</oboInOwl:id>
        <rdfs:label>Harod Valley Region</rdfs:label>
    </owl:NamedIndividual>
    


    <!-- http://purl.obolibrary.org/obo/GAZ_00078188 -->

    <owl:NamedIndividual rdf:about="http://purl.obolibrary.org/obo/GAZ_00078188">
        <obo:RO_0001025 rdf:resource="http://purl.obolibrary.org/obo/GAZ_02000667"/>
        <oboInOwl:hasOBONamespace>GAZ</oboInOwl:hasOBONamespace>
        <oboInOwl:id>GAZ:00078188</oboInOwl:id>
        <rdfs:label>Yizre&apos;el Basin Region</rdfs:label>
    </owl:NamedIndividual>
    


    <!-- http://purl.obolibrary.org/obo/GAZ_00078189 -->

    <owl:NamedIndividual rdf:about="http://purl.obolibrary.org/obo/GAZ_00078189">
        <obo:RO_0001025 rdf:resource="http://purl.obolibrary.org/obo/GAZ_02000667"/>
        <oboInOwl:hasOBONamespace>GAZ</oboInOwl:hasOBONamespace>
        <oboInOwl:id>GAZ:00078189</oboInOwl:id>
        <rdfs:label>Kokhav Plateau Region</rdfs:label>
    </owl:NamedIndividual>
    


    <!-- http://purl.obolibrary.org/obo/GAZ_00078190 -->

    <owl:NamedIndividual rdf:about="http://purl.obolibrary.org/obo/GAZ_00078190">
        <obo:RO_0001025 rdf:resource="http://purl.obolibrary.org/obo/GAZ_02000667"/>
        <oboInOwl:hasOBONamespace>GAZ</oboInOwl:hasOBONamespace>
        <oboInOwl:id>GAZ:00078190</oboInOwl:id>
        <rdfs:label>Nazareth-Tir&apos;an Mountains Region</rdfs:label>
    </owl:NamedIndividual>
    


    <!-- http://purl.obolibrary.org/obo/GAZ_00078191 -->

    <owl:NamedIndividual rdf:about="http://purl.obolibrary.org/obo/GAZ_00078191">
        <obo:RO_0001025 rdf:resource="http://purl.obolibrary.org/obo/GAZ_02000664"/>
        <oboInOwl:hasOBONamespace>GAZ</oboInOwl:hasOBONamespace>
        <oboInOwl:id>GAZ:00078191</oboInOwl:id>
        <rdfs:label>Yehi&apos;am Region</rdfs:label>
    </owl:NamedIndividual>
    


    <!-- http://purl.obolibrary.org/obo/GAZ_00078192 -->

    <owl:NamedIndividual rdf:about="http://purl.obolibrary.org/obo/GAZ_00078192">
        <obo:RO_0001025 rdf:resource="http://purl.obolibrary.org/obo/GAZ_02000664"/>
        <oboInOwl:hasOBONamespace>GAZ</oboInOwl:hasOBONamespace>
        <oboInOwl:id>GAZ:00078192</oboInOwl:id>
        <rdfs:label>Karmi&apos;el Region</rdfs:label>
    </owl:NamedIndividual>
    


    <!-- http://purl.obolibrary.org/obo/GAZ_00078193 -->

    <owl:NamedIndividual rdf:about="http://purl.obolibrary.org/obo/GAZ_00078193">
        <obo:RO_0001025 rdf:resource="http://purl.obolibrary.org/obo/GAZ_02000664"/>
        <oboInOwl:hasOBONamespace>GAZ</oboInOwl:hasOBONamespace>
        <oboInOwl:id>GAZ:00078193</oboInOwl:id>
        <rdfs:label>Shefar&apos;am Region</rdfs:label>
    </owl:NamedIndividual>
    


    <!-- http://purl.obolibrary.org/obo/GAZ_00078194 -->

    <owl:NamedIndividual rdf:about="http://purl.obolibrary.org/obo/GAZ_00078194">
        <obo:RO_0001025 rdf:resource="http://purl.obolibrary.org/obo/GAZ_02000664"/>
        <oboInOwl:hasOBONamespace>GAZ</oboInOwl:hasOBONamespace>
        <oboInOwl:id>GAZ:00078194</oboInOwl:id>
        <rdfs:label>Nahariyya Region</rdfs:label>
    </owl:NamedIndividual>
    


    <!-- http://purl.obolibrary.org/obo/GAZ_00078195 -->

    <owl:NamedIndividual rdf:about="http://purl.obolibrary.org/obo/GAZ_00078195">
        <obo:RO_0001025 rdf:resource="http://purl.obolibrary.org/obo/GAZ_02000664"/>
        <oboInOwl:hasOBONamespace>GAZ</oboInOwl:hasOBONamespace>
        <oboInOwl:id>GAZ:00078195</oboInOwl:id>
        <rdfs:label>Elon Region</rdfs:label>
    </owl:NamedIndividual>
    


    <!-- http://purl.obolibrary.org/obo/GAZ_00078196 -->

    <owl:NamedIndividual rdf:about="http://purl.obolibrary.org/obo/GAZ_00078196">
        <obo:RO_0001025 rdf:resource="http://purl.obolibrary.org/obo/GAZ_02000664"/>
        <oboInOwl:hasOBONamespace>GAZ</oboInOwl:hasOBONamespace>
        <oboInOwl:id>GAZ:00078196</oboInOwl:id>
        <rdfs:label>Akko Region</rdfs:label>
    </owl:NamedIndividual>
    


    <!-- http://purl.obolibrary.org/obo/GAZ_00078197 -->

    <owl:NamedIndividual rdf:about="http://purl.obolibrary.org/obo/GAZ_00078197">
        <obo:RO_0001025 rdf:resource="http://purl.obolibrary.org/obo/GAZ_02000666"/>
        <oboInOwl:hasOBONamespace>GAZ</oboInOwl:hasOBONamespace>
        <oboInOwl:id>GAZ:00078197</oboInOwl:id>
        <rdfs:label>Southern Golan Region</rdfs:label>
    </owl:NamedIndividual>
    


    <!-- http://purl.obolibrary.org/obo/GAZ_00078198 -->

    <owl:NamedIndividual rdf:about="http://purl.obolibrary.org/obo/GAZ_00078198">
        <obo:RO_0001025 rdf:resource="http://purl.obolibrary.org/obo/GAZ_02000666"/>
        <oboInOwl:hasOBONamespace>GAZ</oboInOwl:hasOBONamespace>
        <oboInOwl:id>GAZ:00078198</oboInOwl:id>
        <rdfs:label>Northern Golan Region</rdfs:label>
    </owl:NamedIndividual>
    


    <!-- http://purl.obolibrary.org/obo/GAZ_00078199 -->

    <owl:NamedIndividual rdf:about="http://purl.obolibrary.org/obo/GAZ_00078199">
        <obo:RO_0001025 rdf:resource="http://purl.obolibrary.org/obo/GAZ_02000666"/>
        <oboInOwl:hasOBONamespace>GAZ</oboInOwl:hasOBONamespace>
        <oboInOwl:id>GAZ:00078199</oboInOwl:id>
        <rdfs:label>Hermon Region</rdfs:label>
    </owl:NamedIndividual>
    


    <!-- http://purl.obolibrary.org/obo/GAZ_00078200 -->

    <owl:NamedIndividual rdf:about="http://purl.obolibrary.org/obo/GAZ_00078200">
        <obo:RO_0001025 rdf:resource="http://purl.obolibrary.org/obo/GAZ_02000666"/>
        <oboInOwl:hasOBONamespace>GAZ</oboInOwl:hasOBONamespace>
        <oboInOwl:id>GAZ:00078200</oboInOwl:id>
        <rdfs:label>Middle Golan Region</rdfs:label>
    </owl:NamedIndividual>
    


    <!-- http://purl.obolibrary.org/obo/GAZ_00078201 -->

    <owl:NamedIndividual rdf:about="http://purl.obolibrary.org/obo/GAZ_00078201">
        <obo:RO_0001025 rdf:resource="http://purl.obolibrary.org/obo/GAZ_02000669"/>
        <oboInOwl:hasOBONamespace>GAZ</oboInOwl:hasOBONamespace>
        <oboInOwl:id>GAZ:00078201</oboInOwl:id>
        <rdfs:label>Haifa Region</rdfs:label>
    </owl:NamedIndividual>
    


    <!-- http://purl.obolibrary.org/obo/GAZ_00078202 -->

    <owl:NamedIndividual rdf:about="http://purl.obolibrary.org/obo/GAZ_00078202">
        <obo:RO_0001025 rdf:resource="http://purl.obolibrary.org/obo/GAZ_02000668"/>
        <oboInOwl:hasOBONamespace>GAZ</oboInOwl:hasOBONamespace>
        <oboInOwl:id>GAZ:00078202</oboInOwl:id>
        <rdfs:label>Zikhron Ya&apos;aqov Region</rdfs:label>
    </owl:NamedIndividual>
    


    <!-- http://purl.obolibrary.org/obo/GAZ_00078203 -->

    <owl:NamedIndividual rdf:about="http://purl.obolibrary.org/obo/GAZ_00078203">
        <obo:RO_0001025 rdf:resource="http://purl.obolibrary.org/obo/GAZ_02000668"/>
        <oboInOwl:hasOBONamespace>GAZ</oboInOwl:hasOBONamespace>
        <oboInOwl:id>GAZ:00078203</oboInOwl:id>
        <rdfs:label>Hadera Region</rdfs:label>
    </owl:NamedIndividual>
    


    <!-- http://purl.obolibrary.org/obo/GAZ_00078204 -->

    <owl:NamedIndividual rdf:about="http://purl.obolibrary.org/obo/GAZ_00078204">
        <obo:RO_0001025 rdf:resource="http://purl.obolibrary.org/obo/GAZ_02000668"/>
        <oboInOwl:hasOBONamespace>GAZ</oboInOwl:hasOBONamespace>
        <oboInOwl:id>GAZ:00078204</oboInOwl:id>
        <rdfs:label>Karmel Coast Region</rdfs:label>
    </owl:NamedIndividual>
    


    <!-- http://purl.obolibrary.org/obo/GAZ_00078205 -->

    <owl:NamedIndividual rdf:about="http://purl.obolibrary.org/obo/GAZ_00078205">
        <obo:RO_0001025 rdf:resource="http://purl.obolibrary.org/obo/GAZ_02000668"/>
        <oboInOwl:hasOBONamespace>GAZ</oboInOwl:hasOBONamespace>
        <oboInOwl:id>GAZ:00078205</oboInOwl:id>
        <rdfs:label>Alexander Mountain Region</rdfs:label>
    </owl:NamedIndividual>
    


    <!-- http://purl.obolibrary.org/obo/GAZ_00078206 -->

    <owl:NamedIndividual rdf:about="http://purl.obolibrary.org/obo/GAZ_00078206">
        <obo:RO_0001025 rdf:resource="http://purl.obolibrary.org/obo/GAZ_02000662"/>
        <oboInOwl:hasOBONamespace>GAZ</oboInOwl:hasOBONamespace>
        <oboInOwl:id>GAZ:00078206</oboInOwl:id>
        <rdfs:label>Eastern Sharon</rdfs:label>
    </owl:NamedIndividual>
    


    <!-- http://purl.obolibrary.org/obo/GAZ_00078207 -->

    <owl:NamedIndividual rdf:about="http://purl.obolibrary.org/obo/GAZ_00078207">
        <obo:RO_0001025 rdf:resource="http://purl.obolibrary.org/obo/GAZ_02000662"/>
        <oboInOwl:hasOBONamespace>GAZ</oboInOwl:hasOBONamespace>
        <oboInOwl:id>GAZ:00078207</oboInOwl:id>
        <rdfs:label>Western Sharon</rdfs:label>
    </owl:NamedIndividual>
    


    <!-- http://purl.obolibrary.org/obo/GAZ_00078208 -->

    <owl:NamedIndividual rdf:about="http://purl.obolibrary.org/obo/GAZ_00078208">
        <obo:RO_0001025 rdf:resource="http://purl.obolibrary.org/obo/GAZ_02000660"/>
        <oboInOwl:hasOBONamespace>GAZ</oboInOwl:hasOBONamespace>
        <oboInOwl:id>GAZ:00078208</oboInOwl:id>
        <rdfs:label>Petah Tiqwa Region</rdfs:label>
    </owl:NamedIndividual>
    


    <!-- http://purl.obolibrary.org/obo/GAZ_00078209 -->

    <owl:NamedIndividual rdf:about="http://purl.obolibrary.org/obo/GAZ_00078209">
        <obo:RO_0001025 rdf:resource="http://purl.obolibrary.org/obo/GAZ_02000660"/>
        <oboInOwl:hasOBONamespace>GAZ</oboInOwl:hasOBONamespace>
        <oboInOwl:id>GAZ:00078209</oboInOwl:id>
        <rdfs:label>Southern Sharon Region</rdfs:label>
    </owl:NamedIndividual>
    


    <!-- http://purl.obolibrary.org/obo/GAZ_00078210 -->

    <owl:NamedIndividual rdf:about="http://purl.obolibrary.org/obo/GAZ_00078210">
        <obo:RO_0001025 rdf:resource="http://purl.obolibrary.org/obo/GAZ_02000659"/>
        <oboInOwl:hasOBONamespace>GAZ</oboInOwl:hasOBONamespace>
        <oboInOwl:id>GAZ:00078210</oboInOwl:id>
        <rdfs:label>Lod Region</rdfs:label>
    </owl:NamedIndividual>
    


    <!-- http://purl.obolibrary.org/obo/GAZ_00078211 -->

    <owl:NamedIndividual rdf:about="http://purl.obolibrary.org/obo/GAZ_00078211">
        <obo:RO_0001025 rdf:resource="http://purl.obolibrary.org/obo/GAZ_02000661"/>
        <oboInOwl:hasOBONamespace>GAZ</oboInOwl:hasOBONamespace>
        <oboInOwl:id>GAZ:00078211</oboInOwl:id>
        <rdfs:label>Rehovot Region</rdfs:label>
    </owl:NamedIndividual>
    


    <!-- http://purl.obolibrary.org/obo/GAZ_00078212 -->

    <owl:NamedIndividual rdf:about="http://purl.obolibrary.org/obo/GAZ_00078212">
        <obo:RO_0001025 rdf:resource="http://purl.obolibrary.org/obo/GAZ_02000661"/>
        <oboInOwl:hasOBONamespace>GAZ</oboInOwl:hasOBONamespace>
        <oboInOwl:id>GAZ:00078212</oboInOwl:id>
        <rdfs:label>Rishon LeZiyyon Region</rdfs:label>
    </owl:NamedIndividual>
    


    <!-- http://purl.obolibrary.org/obo/GAZ_00078213 -->

    <owl:NamedIndividual rdf:about="http://purl.obolibrary.org/obo/GAZ_00078213">
        <obo:RO_0001025 rdf:resource="http://purl.obolibrary.org/obo/GAZ_00002709"/>
        <oboInOwl:hasOBONamespace>GAZ</oboInOwl:hasOBONamespace>
        <oboInOwl:id>GAZ:00078213</oboInOwl:id>
        <rdfs:label>Tel Aviv Subdistrict</rdfs:label>
    </owl:NamedIndividual>
    


    <!-- http://purl.obolibrary.org/obo/GAZ_00078214 -->

    <owl:NamedIndividual rdf:about="http://purl.obolibrary.org/obo/GAZ_00078214">
        <obo:RO_0001025 rdf:resource="http://purl.obolibrary.org/obo/GAZ_00078213"/>
        <oboInOwl:hasOBONamespace>GAZ</oboInOwl:hasOBONamespace>
        <oboInOwl:id>GAZ:00078214</oboInOwl:id>
        <rdfs:label>Ramat Gan Region</rdfs:label>
    </owl:NamedIndividual>
    


    <!-- http://purl.obolibrary.org/obo/GAZ_00078215 -->

    <owl:NamedIndividual rdf:about="http://purl.obolibrary.org/obo/GAZ_00078215">
        <obo:RO_0001025 rdf:resource="http://purl.obolibrary.org/obo/GAZ_00078213"/>
        <oboInOwl:hasOBONamespace>GAZ</oboInOwl:hasOBONamespace>
        <oboInOwl:id>GAZ:00078215</oboInOwl:id>
        <rdfs:label>Holon Region</rdfs:label>
    </owl:NamedIndividual>
    


    <!-- http://purl.obolibrary.org/obo/GAZ_00078216 -->

    <owl:NamedIndividual rdf:about="http://purl.obolibrary.org/obo/GAZ_00078216">
        <obo:RO_0001025 rdf:resource="http://purl.obolibrary.org/obo/GAZ_00078213"/>
        <oboInOwl:hasOBONamespace>GAZ</oboInOwl:hasOBONamespace>
        <oboInOwl:id>GAZ:00078216</oboInOwl:id>
        <rdfs:label>Tel Aviv Region</rdfs:label>
    </owl:NamedIndividual>
    


    <!-- http://purl.obolibrary.org/obo/GAZ_00078217 -->

    <owl:NamedIndividual rdf:about="http://purl.obolibrary.org/obo/GAZ_00078217">
        <obo:RO_0001025 rdf:resource="http://purl.obolibrary.org/obo/GAZ_02000671"/>
        <oboInOwl:hasOBONamespace>GAZ</oboInOwl:hasOBONamespace>
        <oboInOwl:id>GAZ:00078217</oboInOwl:id>
        <rdfs:label>Mal&apos;akhi Region</rdfs:label>
    </owl:NamedIndividual>
    


    <!-- http://purl.obolibrary.org/obo/GAZ_00078218 -->

    <owl:NamedIndividual rdf:about="http://purl.obolibrary.org/obo/GAZ_00078218">
        <obo:RO_0001025 rdf:resource="http://purl.obolibrary.org/obo/GAZ_02000671"/>
        <oboInOwl:hasOBONamespace>GAZ</oboInOwl:hasOBONamespace>
        <oboInOwl:id>GAZ:00078218</oboInOwl:id>
        <rdfs:label>Lakhish Region</rdfs:label>
    </owl:NamedIndividual>
    


    <!-- http://purl.obolibrary.org/obo/GAZ_00078219 -->

    <owl:NamedIndividual rdf:about="http://purl.obolibrary.org/obo/GAZ_00078219">
        <obo:RO_0001025 rdf:resource="http://purl.obolibrary.org/obo/GAZ_02000671"/>
        <oboInOwl:hasOBONamespace>GAZ</oboInOwl:hasOBONamespace>
        <oboInOwl:id>GAZ:00078219</oboInOwl:id>
        <rdfs:label>Ashqelon Region</rdfs:label>
    </owl:NamedIndividual>
    


    <!-- http://purl.obolibrary.org/obo/GAZ_00078220 -->

    <owl:NamedIndividual rdf:about="http://purl.obolibrary.org/obo/GAZ_00078220">
        <obo:RO_0001025 rdf:resource="http://purl.obolibrary.org/obo/GAZ_02000671"/>
        <oboInOwl:hasOBONamespace>GAZ</oboInOwl:hasOBONamespace>
        <oboInOwl:id>GAZ:00078220</oboInOwl:id>
        <rdfs:label>Ashdod Region</rdfs:label>
    </owl:NamedIndividual>
    


    <!-- http://purl.obolibrary.org/obo/GAZ_00078221 -->

    <owl:NamedIndividual rdf:about="http://purl.obolibrary.org/obo/GAZ_00078221">
        <obo:RO_0001025 rdf:resource="http://purl.obolibrary.org/obo/GAZ_02000670"/>
        <oboInOwl:hasOBONamespace>GAZ</oboInOwl:hasOBONamespace>
        <oboInOwl:id>GAZ:00078221</oboInOwl:id>
        <rdfs:label>Dead Sea Region</rdfs:label>
    </owl:NamedIndividual>
    


    <!-- http://purl.obolibrary.org/obo/GAZ_00078222 -->

    <owl:NamedIndividual rdf:about="http://purl.obolibrary.org/obo/GAZ_00078222">
        <obo:RO_0001025 rdf:resource="http://purl.obolibrary.org/obo/GAZ_02000670"/>
        <oboInOwl:hasOBONamespace>GAZ</oboInOwl:hasOBONamespace>
        <oboInOwl:id>GAZ:00078222</oboInOwl:id>
        <rdfs:label>Southern Negev Mountain Region</rdfs:label>
    </owl:NamedIndividual>
    


    <!-- http://purl.obolibrary.org/obo/GAZ_00078223 -->

    <owl:NamedIndividual rdf:about="http://purl.obolibrary.org/obo/GAZ_00078223">
        <obo:RO_0001025 rdf:resource="http://purl.obolibrary.org/obo/GAZ_02000670"/>
        <oboInOwl:hasOBONamespace>GAZ</oboInOwl:hasOBONamespace>
        <oboInOwl:id>GAZ:00078223</oboInOwl:id>
        <rdfs:label>Gerar Region</rdfs:label>
    </owl:NamedIndividual>
    


    <!-- http://purl.obolibrary.org/obo/GAZ_00078224 -->

    <owl:NamedIndividual rdf:about="http://purl.obolibrary.org/obo/GAZ_00078224">
        <obo:RO_0001025 rdf:resource="http://purl.obolibrary.org/obo/GAZ_02000670"/>
        <oboInOwl:hasOBONamespace>GAZ</oboInOwl:hasOBONamespace>
        <oboInOwl:id>GAZ:00078224</oboInOwl:id>
        <rdfs:label>Arava Region</rdfs:label>
    </owl:NamedIndividual>
    


    <!-- http://purl.obolibrary.org/obo/GAZ_00078225 -->

    <owl:NamedIndividual rdf:about="http://purl.obolibrary.org/obo/GAZ_00078225">
        <obo:RO_0001025 rdf:resource="http://purl.obolibrary.org/obo/GAZ_02000670"/>
        <oboInOwl:hasOBONamespace>GAZ</oboInOwl:hasOBONamespace>
        <oboInOwl:id>GAZ:00078225</oboInOwl:id>
        <rdfs:label>Northern Negev Mountain Region</rdfs:label>
    </owl:NamedIndividual>
    


    <!-- http://purl.obolibrary.org/obo/GAZ_00078226 -->

    <owl:NamedIndividual rdf:about="http://purl.obolibrary.org/obo/GAZ_00078226">
        <obo:RO_0001025 rdf:resource="http://purl.obolibrary.org/obo/GAZ_02000670"/>
        <oboInOwl:hasOBONamespace>GAZ</oboInOwl:hasOBONamespace>
        <oboInOwl:id>GAZ:00078226</oboInOwl:id>
        <rdfs:label>Be&apos;er Sheva Region</rdfs:label>
    </owl:NamedIndividual>
    


    <!-- http://purl.obolibrary.org/obo/GAZ_00078227 -->

    <owl:NamedIndividual rdf:about="http://purl.obolibrary.org/obo/GAZ_00078227">
        <obo:RO_0001025 rdf:resource="http://purl.obolibrary.org/obo/GAZ_02000670"/>
        <oboInOwl:hasOBONamespace>GAZ</oboInOwl:hasOBONamespace>
        <oboInOwl:id>GAZ:00078227</oboInOwl:id>
        <rdfs:label>Besor Region</rdfs:label>
    </owl:NamedIndividual>
    


    <!-- http://purl.obolibrary.org/obo/GAZ_00078228 -->

    <owl:NamedIndividual rdf:about="http://purl.obolibrary.org/obo/GAZ_00078228">
        <obo:RO_0001025 rdf:resource="http://purl.obolibrary.org/obo/GAZ_00002711"/>
        <obo:IAO_0000115>A regional council in the Haifa District.</obo:IAO_0000115>
        <oboInOwl:hasOBONamespace>GAZ</oboInOwl:hasOBONamespace>
        <oboInOwl:id>GAZ:00078228</oboInOwl:id>
        <rdfs:label>Zevulun Regional Council</rdfs:label>
    </owl:NamedIndividual>
    


    <!-- http://purl.obolibrary.org/obo/GAZ_00078229 -->

    <owl:NamedIndividual rdf:about="http://purl.obolibrary.org/obo/GAZ_00078229">
        <obo:RO_0001025 rdf:resource="http://purl.obolibrary.org/obo/GAZ_00002711"/>
        <obo:IAO_0000115>A regional council located in the northern Israeli Coastal Plain. The council serves a large area, from Tirat HaCarmel in the north to Caesarea in the south and its offices are located in Ein HaCarmel, south of Haifa.</obo:IAO_0000115>
        <oboInOwl:hasOBONamespace>GAZ</oboInOwl:hasOBONamespace>
        <oboInOwl:id>GAZ:00078229</oboInOwl:id>
        <rdfs:label>Hof HaCarmel Regional Council</rdfs:label>
    </owl:NamedIndividual>
    


    <!-- http://purl.obolibrary.org/obo/GAZ_00078230 -->

    <owl:NamedIndividual rdf:about="http://purl.obolibrary.org/obo/GAZ_00078230">
        <obo:RO_0001025 rdf:resource="http://purl.obolibrary.org/obo/GAZ_00002711"/>
        <obo:IAO_0000115>A regional council in the Haifa District.</obo:IAO_0000115>
        <oboInOwl:hasOBONamespace>GAZ</oboInOwl:hasOBONamespace>
        <oboInOwl:id>GAZ:00078230</oboInOwl:id>
        <rdfs:label>Alona Regional Council</rdfs:label>
    </owl:NamedIndividual>
    


    <!-- http://purl.obolibrary.org/obo/GAZ_00078231 -->

    <owl:NamedIndividual rdf:about="http://purl.obolibrary.org/obo/GAZ_00078231">
        <obo:RO_0001025 rdf:resource="http://purl.obolibrary.org/obo/GAZ_00002710"/>
        <obo:IAO_0000115>A regional council in the northwestern Negev desert in Israel.</obo:IAO_0000115>
        <oboInOwl:hasOBONamespace>GAZ</oboInOwl:hasOBONamespace>
        <oboInOwl:id>GAZ:00078231</oboInOwl:id>
        <rdfs:label>Abu Basma Regional Council</rdfs:label>
    </owl:NamedIndividual>
    


    <!-- http://purl.obolibrary.org/obo/GAZ_00078232 -->

    <owl:NamedIndividual rdf:about="http://purl.obolibrary.org/obo/GAZ_00078232">
        <obo:RO_0001025 rdf:resource="http://purl.obolibrary.org/obo/GAZ_00002710"/>
        <obo:IAO_0000115>A regional council in the northern Negev in the south of Israel. Most of its territory lies north of Beersheba and the rest bounds Beersheba on the west and east sides as well. The eastern border of this territory straddles the Green Line.</obo:IAO_0000115>
        <oboInOwl:hasOBONamespace>GAZ</oboInOwl:hasOBONamespace>
        <oboInOwl:id>GAZ:00078232</oboInOwl:id>
        <rdfs:label>Bnei Shimon Regional Council</rdfs:label>
    </owl:NamedIndividual>
    


    <!-- http://purl.obolibrary.org/obo/GAZ_00078233 -->

    <owl:NamedIndividual rdf:about="http://purl.obolibrary.org/obo/GAZ_00078233">
        <obo:RO_0001025 rdf:resource="http://purl.obolibrary.org/obo/GAZ_00002710"/>
        <obo:IAO_0000115>A Regional Council in the South District of Israel. It encompasses 7 or 8 settlements near the eastern border of Israel, south of the Dead Sea. All settlements are located near Route 90, which is the longest north-south road in Israel.</obo:IAO_0000115>
        <oboInOwl:hasOBONamespace>GAZ</oboInOwl:hasOBONamespace>
        <oboInOwl:id>GAZ:00078233</oboInOwl:id>
        <rdfs:label>Central Arava Regional Council</rdfs:label>
    </owl:NamedIndividual>
    


    <!-- http://purl.obolibrary.org/obo/GAZ_00078234 -->

    <owl:NamedIndividual rdf:about="http://purl.obolibrary.org/obo/GAZ_00078234">
        <obo:RO_0001025 rdf:resource="http://purl.obolibrary.org/obo/GAZ_00002710"/>
        <obo:IAO_0000115>A regional council in the South District of Israel, near the city of Eilat. It is the southernmost regional council in Israel.</obo:IAO_0000115>
        <oboInOwl:hasOBONamespace>GAZ</oboInOwl:hasOBONamespace>
        <oboInOwl:id>GAZ:00078234</oboInOwl:id>
        <rdfs:label>Hevel Eilot Regional Council</rdfs:label>
    </owl:NamedIndividual>
    


    <!-- http://purl.obolibrary.org/obo/GAZ_00078235 -->

    <owl:NamedIndividual rdf:about="http://purl.obolibrary.org/obo/GAZ_00078235">
        <obo:RO_0001025 rdf:resource="http://purl.obolibrary.org/obo/GAZ_00078234"/>
        <obo:IAO_0000115>A park located about 30 km north of Eilat, Israel.</obo:IAO_0000115>
        <oboInOwl:hasOBONamespace>GAZ</oboInOwl:hasOBONamespace>
        <oboInOwl:id>GAZ:00078235</oboInOwl:id>
        <rdfs:label>Timna Valley Park</rdfs:label>
    </owl:NamedIndividual>
    


    <!-- http://purl.obolibrary.org/obo/GAZ_00078236 -->

    <owl:NamedIndividual rdf:about="http://purl.obolibrary.org/obo/GAZ_00078236">
        <obo:RO_0001025 rdf:resource="http://purl.obolibrary.org/obo/GAZ_00002710"/>
        <obo:IAO_0000115>A Regional Council in the Southern District if Israel.</obo:IAO_0000115>
        <oboInOwl:hasOBONamespace>GAZ</oboInOwl:hasOBONamespace>
        <oboInOwl:id>GAZ:00078236</oboInOwl:id>
        <rdfs:label>Hof Ashkelon Regional Council</rdfs:label>
    </owl:NamedIndividual>
    


    <!-- http://purl.obolibrary.org/obo/GAZ_00078237 -->

    <owl:NamedIndividual rdf:about="http://purl.obolibrary.org/obo/GAZ_00078237">
        <obo:RO_0001025 rdf:resource="http://purl.obolibrary.org/obo/GAZ_00078218"/>
        <obo:IAO_0000115>A regional council in the South District of Israel. It surrounds the ancient city of Lakhish and the modern city of Kiryat Gat.</obo:IAO_0000115>
        <oboInOwl:hasOBONamespace>GAZ</oboInOwl:hasOBONamespace>
        <oboInOwl:id>GAZ:00078237</oboInOwl:id>
        <rdfs:label>Lakhish Regional Council</rdfs:label>
    </owl:NamedIndividual>
    


    <!-- http://purl.obolibrary.org/obo/GAZ_00078238 -->

    <owl:NamedIndividual rdf:about="http://purl.obolibrary.org/obo/GAZ_00078238">
        <obo:RO_0001025 rdf:resource="http://purl.obolibrary.org/obo/GAZ_00002710"/>
        <obo:IAO_0000115>A Regional Council in the South District of Israel.</obo:IAO_0000115>
        <oboInOwl:hasOBONamespace>GAZ</oboInOwl:hasOBONamespace>
        <oboInOwl:id>GAZ:00078238</oboInOwl:id>
        <rdfs:label>Merhavim Regional Council</rdfs:label>
    </owl:NamedIndividual>
    


    <!-- http://purl.obolibrary.org/obo/GAZ_00078239 -->

    <owl:NamedIndividual rdf:about="http://purl.obolibrary.org/obo/GAZ_00078239">
        <obo:RO_0001025 rdf:resource="http://purl.obolibrary.org/obo/GAZ_00002710"/>
        <obo:IAO_0000115>A regional council in the Negev desert in Israel. The largest regional council in the country, its headquarters are located on Highway 40 between Mashabei Sadeh and Tlalim.</obo:IAO_0000115>
        <oboInOwl:hasOBONamespace>GAZ</oboInOwl:hasOBONamespace>
        <oboInOwl:id>GAZ:00078239</oboInOwl:id>
        <rdfs:label>Ramat HaNegev Regional Council</rdfs:label>
    </owl:NamedIndividual>
    


    <!-- http://purl.obolibrary.org/obo/GAZ_00078240 -->

    <owl:NamedIndividual rdf:about="http://purl.obolibrary.org/obo/GAZ_00078240">
        <obo:RO_0001025 rdf:resource="http://purl.obolibrary.org/obo/GAZ_00002710"/>
        <obo:IAO_0000115>A regional council in the north-western Negev, in Israel&apos;s Southern District. The Regional Council&apos;s territory lies midway between Beersheba and Ashkelon, bounded on the west by the Gaza Strip. The eastern border abuts Bnei Shimon. The city of Sderot forms an enclave within Sha&apos;ar HaNegev.</obo:IAO_0000115>
        <oboInOwl:hasOBONamespace>GAZ</oboInOwl:hasOBONamespace>
        <oboInOwl:id>GAZ:00078240</oboInOwl:id>
        <rdfs:label>Sha&apos;ar HaNegev Regional Council</rdfs:label>
    </owl:NamedIndividual>
    


    <!-- http://purl.obolibrary.org/obo/GAZ_00078241 -->

    <owl:NamedIndividual rdf:about="http://purl.obolibrary.org/obo/GAZ_00078241">
        <obo:RO_0001025 rdf:resource="http://purl.obolibrary.org/obo/GAZ_00002710"/>
        <obo:IAO_0000115>A regional council in southern Israel near the city of Kiryat Gat. The council is bordered on the north by the Be&apos;er Tuvia Regional Council, on the east by Yoav Regional Council and Kiryat Gat, on the south by Lakhish Regional Council, and on the west by Hof Ashkelon Regional Council, Yoav Regional Council.</obo:IAO_0000115>
        <oboInOwl:hasOBONamespace>GAZ</oboInOwl:hasOBONamespace>
        <oboInOwl:id>GAZ:00078241</oboInOwl:id>
        <rdfs:label>Shafir Regional Council</rdfs:label>
    </owl:NamedIndividual>
    


    <!-- http://purl.obolibrary.org/obo/GAZ_00078242 -->

    <owl:NamedIndividual rdf:about="http://purl.obolibrary.org/obo/GAZ_00078242">
        <obo:RO_0001025 rdf:resource="http://purl.obolibrary.org/obo/GAZ_00002710"/>
        <obo:IAO_0000115>A regional council in Israel&apos;s South District, on the south and western edges of the Dead Sea along the Arava valley.</obo:IAO_0000115>
        <oboInOwl:hasOBONamespace>GAZ</oboInOwl:hasOBONamespace>
        <oboInOwl:id>GAZ:00078242</oboInOwl:id>
        <rdfs:label>Tamar Regional Council</rdfs:label>
    </owl:NamedIndividual>
    


    <!-- http://purl.obolibrary.org/obo/GAZ_00078243 -->

    <owl:NamedIndividual rdf:about="http://purl.obolibrary.org/obo/GAZ_00078243">
        <obo:RO_0001025 rdf:resource="http://purl.obolibrary.org/obo/GAZ_00002710"/>
        <obo:IAO_0000115>A regional council in the South District of Israel. It is located near the cities of Kiryat Gat, Kiryat Malakhi and Ashkelon. The council contains two parts which are not contiguous geographically. The main part is bordered on the north by Nahal Sorek Regional Council, on the west by Be&apos;er Tuvia Regional Council and Shafir Regional Council, on the south by Lakhish Regional Council and Kiryat Gat, and on the east by Matte Yehuda Regional Council. The western portion of the council, which includes the kibbutzim Negba and Sde Yoav, is bordered on the north and east by Shafir Regional Council, on the west by Hof Ashkelon Regional Council, and on the west by Lakhish Regional Council.</obo:IAO_0000115>
        <oboInOwl:hasOBONamespace>GAZ</oboInOwl:hasOBONamespace>
        <oboInOwl:id>GAZ:00078243</oboInOwl:id>
        <rdfs:label>Yoav Regional Council</rdfs:label>
    </owl:NamedIndividual>
    


    <!-- http://purl.obolibrary.org/obo/GAZ_00078244 -->

    <owl:NamedIndividual rdf:about="http://purl.obolibrary.org/obo/GAZ_00078244">
        <obo:RO_0001025 rdf:resource="http://purl.obolibrary.org/obo/GAZ_00002710"/>
        <obo:IAO_0000115>A Bedouin town (local council) in the South District of Israel.</obo:IAO_0000115>
        <oboInOwl:hasOBONamespace>GAZ</oboInOwl:hasOBONamespace>
        <oboInOwl:id>GAZ:00078244</oboInOwl:id>
        <rdfs:label>Ar&apos;arat an-Naqab Local Council</rdfs:label>
    </owl:NamedIndividual>
    


    <!-- http://purl.obolibrary.org/obo/GAZ_00078245 -->

    <owl:NamedIndividual rdf:about="http://purl.obolibrary.org/obo/GAZ_00078245">
        <rdf:type rdf:resource="http://purl.obolibrary.org/obo/ENVO_00000856"/>
        <obo:RO_0001025 rdf:resource="http://purl.obolibrary.org/obo/GAZ_00002710"/>
        <obo:IAO_0000115>A Bedouin village in the South District of Israel. It is located near Beersheba and beside the town Meitar. The village was established in 1990, and was declared a local council in 1996.</obo:IAO_0000115>
        <oboInOwl:hasOBONamespace>GAZ</oboInOwl:hasOBONamespace>
        <oboInOwl:id>GAZ:00078245</oboInOwl:id>
        <rdfs:label>Hura Local Council</rdfs:label>
    </owl:NamedIndividual>
    


    <!-- http://purl.obolibrary.org/obo/GAZ_00078246 -->

    <owl:NamedIndividual rdf:about="http://purl.obolibrary.org/obo/GAZ_00078246">
        <obo:RO_0001025 rdf:resource="http://purl.obolibrary.org/obo/GAZ_00002710"/>
        <obo:IAO_0000115>A Bedouin town (local council) in the Southern District of Israel.</obo:IAO_0000115>
        <oboInOwl:hasOBONamespace>GAZ</oboInOwl:hasOBONamespace>
        <oboInOwl:id>GAZ:00078246</oboInOwl:id>
        <rdfs:label>Kuseife Local Council</rdfs:label>
    </owl:NamedIndividual>
    


    <!-- http://purl.obolibrary.org/obo/GAZ_00078247 -->

    <owl:NamedIndividual rdf:about="http://purl.obolibrary.org/obo/GAZ_00078247">
        <obo:RO_0001025 rdf:resource="http://purl.obolibrary.org/obo/GAZ_00002710"/>
        <obo:IAO_0000115>A Bedouin town (local council) in the Southern District of Israel.</obo:IAO_0000115>
        <oboInOwl:hasOBONamespace>GAZ</oboInOwl:hasOBONamespace>
        <oboInOwl:id>GAZ:00078247</oboInOwl:id>
        <rdfs:label>Lakiya Local Council</rdfs:label>
    </owl:NamedIndividual>
    


    <!-- http://purl.obolibrary.org/obo/GAZ_00078248 -->

    <owl:NamedIndividual rdf:about="http://purl.obolibrary.org/obo/GAZ_00078248">
        <obo:RO_0001025 rdf:resource="http://purl.obolibrary.org/obo/GAZ_00002710"/>
        <obo:IAO_0000115>A local council in the Southern District of Israel, bordering Be&apos;er Sheva.</obo:IAO_0000115>
        <oboInOwl:hasOBONamespace>GAZ</oboInOwl:hasOBONamespace>
        <oboInOwl:id>GAZ:00078248</oboInOwl:id>
        <rdfs:label>Tel as-Sabi Local Council</rdfs:label>
    </owl:NamedIndividual>
    


    <!-- http://purl.obolibrary.org/obo/GAZ_00078249 -->

    <owl:NamedIndividual rdf:about="http://purl.obolibrary.org/obo/GAZ_00078249">
        <obo:RO_0001025 rdf:resource="http://purl.obolibrary.org/obo/GAZ_00002710"/>
        <obo:IAO_0000115>A local council in the South District of Israel, southeast of Beersheba.</obo:IAO_0000115>
        <oboInOwl:hasOBONamespace>GAZ</oboInOwl:hasOBONamespace>
        <oboInOwl:id>GAZ:00078249</oboInOwl:id>
        <rdfs:label>Shaqib al-Salam Local Council</rdfs:label>
    </owl:NamedIndividual>
    


    <!-- http://purl.obolibrary.org/obo/GAZ_00078250 -->

    <owl:NamedIndividual rdf:about="http://purl.obolibrary.org/obo/GAZ_00078250">
        <obo:RO_0001025 rdf:resource="http://purl.obolibrary.org/obo/GAZ_00002710"/>
        <obo:IAO_0000115>A local Council in the Southern District of Israel, in the northern Negev desert. Founded in 1983, it is located 15 km north of Beersheba and 4 km east of Rahat.</obo:IAO_0000115>
        <oboInOwl:hasOBONamespace>GAZ</oboInOwl:hasOBONamespace>
        <oboInOwl:id>GAZ:00078250</oboInOwl:id>
        <rdfs:label>Lehavim Local Council</rdfs:label>
    </owl:NamedIndividual>
    


    <!-- http://purl.obolibrary.org/obo/GAZ_00078251 -->

    <owl:NamedIndividual rdf:about="http://purl.obolibrary.org/obo/GAZ_00078251">
        <obo:RO_0001025 rdf:resource="http://purl.obolibrary.org/obo/GAZ_00002710"/>
        <obo:IAO_0000115>A local council in the Southern District of Israel, in the Negev desert.</obo:IAO_0000115>
        <oboInOwl:hasOBONamespace>GAZ</oboInOwl:hasOBONamespace>
        <oboInOwl:id>GAZ:00078251</oboInOwl:id>
        <rdfs:label>Yeruham Local Council</rdfs:label>
    </owl:NamedIndividual>
    


    <!-- http://purl.obolibrary.org/obo/GAZ_00078252 -->

    <owl:NamedIndividual rdf:about="http://purl.obolibrary.org/obo/GAZ_00078252">
        <obo:RO_0001025 rdf:resource="http://purl.obolibrary.org/obo/GAZ_00002710"/>
        <obo:IAO_0000115>A local council in the South District of Israel, bordering Beersheba. It is located on Highway 60, between Beersheba and the Shoket Junction.</obo:IAO_0000115>
        <oboInOwl:hasOBONamespace>GAZ</oboInOwl:hasOBONamespace>
        <oboInOwl:id>GAZ:00078252</oboInOwl:id>
        <rdfs:label>Omer Local Council</rdfs:label>
    </owl:NamedIndividual>
    


    <!-- http://purl.obolibrary.org/obo/GAZ_00078253 -->

    <owl:NamedIndividual rdf:about="http://purl.obolibrary.org/obo/GAZ_00078253">
        <obo:RO_0001025 rdf:resource="http://purl.obolibrary.org/obo/GAZ_00002710"/>
        <obo:IAO_0000115>A local council in the Negev desert of southern Israel. It is situated on the northern ridge at an elevation of 800 m overlooking an enormous erosion cirque known as the Ramon Crater.</obo:IAO_0000115>
        <oboInOwl:hasOBONamespace>GAZ</oboInOwl:hasOBONamespace>
        <oboInOwl:id>GAZ:00078253</oboInOwl:id>
        <rdfs:label>Mitzpe Ramon Local Council</rdfs:label>
    </owl:NamedIndividual>
    


    <!-- http://purl.obolibrary.org/obo/GAZ_00078254 -->

    <owl:NamedIndividual rdf:about="http://purl.obolibrary.org/obo/GAZ_00078254">
        <obo:RO_0001025 rdf:resource="http://purl.obolibrary.org/obo/GAZ_00002710"/>
        <obo:IAO_0000115>A small local council north-east of Beersheba, in Israel&apos;s Southern District. The town lies on Highway 60 just south of the Green Line on the southern edge of Mount Hebron, alongside the Yatir Forest.</obo:IAO_0000115>
        <oboInOwl:hasOBONamespace>GAZ</oboInOwl:hasOBONamespace>
        <oboInOwl:id>GAZ:00078254</oboInOwl:id>
        <rdfs:label>Meitar Local Council</rdfs:label>
    </owl:NamedIndividual>
    


    <!-- http://purl.obolibrary.org/obo/GAZ_00078255 -->

    <owl:NamedIndividual rdf:about="http://purl.obolibrary.org/obo/GAZ_00078255">
        <obo:RO_0001025 rdf:resource="http://purl.obolibrary.org/obo/GAZ_00002710"/>
        <obo:IAO_0000115>A man-made forest in Israel, located on the southern slopes of Mount Hebron, on the edge of the Negev Desert.</obo:IAO_0000115>
        <oboInOwl:hasOBONamespace>GAZ</oboInOwl:hasOBONamespace>
        <oboInOwl:id>GAZ:00078255</oboInOwl:id>
        <rdfs:label>Yatir Forest</rdfs:label>
    </owl:NamedIndividual>
    


    <!-- http://purl.obolibrary.org/obo/GAZ_00078256 -->

    <owl:NamedIndividual rdf:about="http://purl.obolibrary.org/obo/GAZ_00078256">
        <obo:RO_0001025 rdf:resource="http://purl.obolibrary.org/obo/GAZ_00002710"/>
        <obo:IAO_0000115>A modern city in the South District of Israel, on the border of the Negev and Judean Deserts. Located 25 km west of the Dead Sea and 45 km east of the city Beersheba.</obo:IAO_0000115>
        <oboInOwl:hasOBONamespace>GAZ</oboInOwl:hasOBONamespace>
        <oboInOwl:id>GAZ:00078256</oboInOwl:id>
        <rdfs:label>City of Arad</rdfs:label>
    </owl:NamedIndividual>
    


    <!-- http://purl.obolibrary.org/obo/GAZ_00078257 -->

    <owl:NamedIndividual rdf:about="http://purl.obolibrary.org/obo/GAZ_00078257">
        <obo:RO_0001025 rdf:resource="http://purl.obolibrary.org/obo/GAZ_00078220"/>
        <obo:IAO_0000115>A city located in the South District of Israel, on the Mediterranean Sea coast.</obo:IAO_0000115>
        <oboInOwl:hasOBONamespace>GAZ</oboInOwl:hasOBONamespace>
        <oboInOwl:id>GAZ:00078257</oboInOwl:id>
        <rdfs:label>City of Ashdod</rdfs:label>
    </owl:NamedIndividual>
    


    <!-- http://purl.obolibrary.org/obo/GAZ_00078258 -->

    <owl:NamedIndividual rdf:about="http://purl.obolibrary.org/obo/GAZ_00078258">
        <obo:RO_0001025 rdf:resource="http://purl.obolibrary.org/obo/GAZ_00078219"/>
        <obo:IAO_0000115>A populated place. A city in the western Negev, in the South District of Israel.</obo:IAO_0000115>
        <oboInOwl:hasOBONamespace>GAZ</oboInOwl:hasOBONamespace>
        <oboInOwl:id>GAZ:00078258</oboInOwl:id>
        <rdfs:label>City of Ashkelon</rdfs:label>
    </owl:NamedIndividual>
    


    <!-- http://purl.obolibrary.org/obo/GAZ_00078259 -->

    <owl:NamedIndividual rdf:about="http://purl.obolibrary.org/obo/GAZ_00078259">
        <obo:RO_0001025 rdf:resource="http://purl.obolibrary.org/obo/GAZ_00078226"/>
        <obo:IAO_0000115>The largest city in the Negev desert of southern Israel. Beersheba is located in the Southern District of the country.</obo:IAO_0000115>
        <oboInOwl:hasOBONamespace>GAZ</oboInOwl:hasOBONamespace>
        <oboInOwl:id>GAZ:00078259</oboInOwl:id>
        <rdfs:label>City of Beersheba</rdfs:label>
    </owl:NamedIndividual>
    


    <!-- http://purl.obolibrary.org/obo/GAZ_00078260 -->

    <owl:NamedIndividual rdf:about="http://purl.obolibrary.org/obo/GAZ_00078260">
        <obo:RO_0001025 rdf:resource="http://purl.obolibrary.org/obo/GAZ_00002710"/>
        <obo:IAO_0000115>An Israeli city in the Negev desert, 36 km to the south of Beersheba and 35 km west of the Dead Sea above the Arava valley in the Southern District of Israel.</obo:IAO_0000115>
        <oboInOwl:hasOBONamespace>GAZ</oboInOwl:hasOBONamespace>
        <oboInOwl:id>GAZ:00078260</oboInOwl:id>
        <rdfs:label>City of Dimona</rdfs:label>
    </owl:NamedIndividual>
    


    <!-- http://purl.obolibrary.org/obo/GAZ_00078261 -->

    <owl:NamedIndividual rdf:about="http://purl.obolibrary.org/obo/GAZ_00078261">
        <obo:RO_0001025 rdf:resource="http://purl.obolibrary.org/obo/GAZ_00002710"/>
        <obo:IAO_0000115>Israel&apos;s southernmost city and is a tourist resort and port located at the northern tip of the Red Sea, on the Gulf of Eilat arm of the Indian Ocean. It is part of the Southern Negev Desert, at the south end of the Arava, and straddles the southern end of the geographic line demarcating Africa from Asia.</obo:IAO_0000115>
        <oboInOwl:hasOBONamespace>GAZ</oboInOwl:hasOBONamespace>
        <oboInOwl:id>GAZ:00078261</oboInOwl:id>
        <rdfs:label>City of Eliat</rdfs:label>
    </owl:NamedIndividual>
    


    <!-- http://purl.obolibrary.org/obo/GAZ_00078262 -->

    <owl:NamedIndividual rdf:about="http://purl.obolibrary.org/obo/GAZ_00078262">
        <obo:RO_0001025 rdf:resource="http://purl.obolibrary.org/obo/GAZ_00002710"/>
        <obo:IAO_0000115>A populated place. A city in the Southern District of Israel. It lies 56 km south of Tel-Aviv, 43 km north of Beersheba and 68 km from Jerusalem.</obo:IAO_0000115>
        <oboInOwl:hasOBONamespace>GAZ</oboInOwl:hasOBONamespace>
        <oboInOwl:id>GAZ:00078262</oboInOwl:id>
        <rdfs:label>City of Kiryat Gat</rdfs:label>
    </owl:NamedIndividual>
    


    <!-- http://purl.obolibrary.org/obo/GAZ_00078263 -->

    <owl:NamedIndividual rdf:about="http://purl.obolibrary.org/obo/GAZ_00078263">
        <obo:RO_0001025 rdf:resource="http://purl.obolibrary.org/obo/GAZ_00002710"/>
        <obo:IAO_0000115>A populated place. A city in Israel&apos;s Southern District, 17 km from Ashkelon.</obo:IAO_0000115>
        <oboInOwl:hasOBONamespace>GAZ</oboInOwl:hasOBONamespace>
        <oboInOwl:id>GAZ:00078263</oboInOwl:id>
        <rdfs:label>City of Kiryat Malakhi</rdfs:label>
    </owl:NamedIndividual>
    


    <!-- http://purl.obolibrary.org/obo/GAZ_00078264 -->

    <owl:NamedIndividual rdf:about="http://purl.obolibrary.org/obo/GAZ_00078264">
        <obo:RO_0001025 rdf:resource="http://purl.obolibrary.org/obo/GAZ_00002710"/>
        <obo:IAO_0000115>A populated place. A city in the Southern District of Israel in Israel.</obo:IAO_0000115>
        <oboInOwl:hasOBONamespace>GAZ</oboInOwl:hasOBONamespace>
        <oboInOwl:id>GAZ:00078264</oboInOwl:id>
        <rdfs:label>City of Ofakim</rdfs:label>
    </owl:NamedIndividual>
    


    <!-- http://purl.obolibrary.org/obo/GAZ_00078265 -->

    <owl:NamedIndividual rdf:about="http://purl.obolibrary.org/obo/GAZ_00078265">
        <obo:RO_0001025 rdf:resource="http://purl.obolibrary.org/obo/GAZ_00002710"/>
        <obo:IAO_0000115>A populated place. A city in the Southern District of Israel in Israel.</obo:IAO_0000115>
        <oboInOwl:hasOBONamespace>GAZ</oboInOwl:hasOBONamespace>
        <oboInOwl:id>GAZ:00078265</oboInOwl:id>
        <rdfs:label>City of Netivot</rdfs:label>
    </owl:NamedIndividual>
    


    <!-- http://purl.obolibrary.org/obo/GAZ_00078266 -->

    <owl:NamedIndividual rdf:about="http://purl.obolibrary.org/obo/GAZ_00078266">
        <obo:RO_0001025 rdf:resource="http://purl.obolibrary.org/obo/GAZ_00002710"/>
        <obo:IAO_0000115>A populated place. A city in the South District of Israel.</obo:IAO_0000115>
        <oboInOwl:hasOBONamespace>GAZ</oboInOwl:hasOBONamespace>
        <oboInOwl:id>GAZ:00078266</oboInOwl:id>
        <rdfs:label>City of Rahat</rdfs:label>
    </owl:NamedIndividual>
    


    <!-- http://purl.obolibrary.org/obo/GAZ_00078267 -->

    <owl:NamedIndividual rdf:about="http://purl.obolibrary.org/obo/GAZ_00078267">
        <obo:RO_0001025 rdf:resource="http://purl.obolibrary.org/obo/GAZ_00002710"/>
        <obo:IAO_0000115>A populated place. A city in the western Negev, in the South District of Israel.</obo:IAO_0000115>
        <oboInOwl:hasOBONamespace>GAZ</oboInOwl:hasOBONamespace>
        <oboInOwl:id>GAZ:00078267</oboInOwl:id>
        <rdfs:label>City of Sderot</rdfs:label>
    </owl:NamedIndividual>
    


    <!-- http://purl.obolibrary.org/obo/GAZ_00078268 -->

    <owl:NamedIndividual rdf:about="http://purl.obolibrary.org/obo/GAZ_00078268">
        <obo:RO_0001025 rdf:resource="http://purl.obolibrary.org/obo/GAZ_00078213"/>
        <obo:IAO_0000115>A local council in the Tel Aviv District of Israel. It is located near the former Arab village of Yazur.</obo:IAO_0000115>
        <oboInOwl:hasOBONamespace>GAZ</oboInOwl:hasOBONamespace>
        <oboInOwl:id>GAZ:00078268</oboInOwl:id>
        <rdfs:label>Azor Local Council</rdfs:label>
    </owl:NamedIndividual>
    


    <!-- http://purl.obolibrary.org/obo/GAZ_00078269 -->

    <owl:NamedIndividual rdf:about="http://purl.obolibrary.org/obo/GAZ_00078269">
        <obo:RO_0001025 rdf:resource="http://purl.obolibrary.org/obo/GAZ_00078213"/>
        <obo:IAO_0000115>A local council in Israel, found in the Tel Aviv District.</obo:IAO_0000115>
        <oboInOwl:hasOBONamespace>GAZ</oboInOwl:hasOBONamespace>
        <oboInOwl:id>GAZ:00078269</oboInOwl:id>
        <rdfs:label>Kfar Shmaryahu Local Council</rdfs:label>
    </owl:NamedIndividual>
    


    <!-- http://purl.obolibrary.org/obo/GAZ_00078270 -->

    <owl:NamedIndividual rdf:about="http://purl.obolibrary.org/obo/GAZ_00078270">
        <obo:RO_0001025 rdf:resource="http://purl.obolibrary.org/obo/GAZ_00078216"/>
        <oboInOwl:hasOBONamespace>GAZ</oboInOwl:hasOBONamespace>
        <oboInOwl:id>GAZ:00078270</oboInOwl:id>
        <rdfs:label>City of Tel Aviv</rdfs:label>
    </owl:NamedIndividual>
    


    <!-- http://purl.obolibrary.org/obo/GAZ_00078271 -->

    <owl:NamedIndividual rdf:about="http://purl.obolibrary.org/obo/GAZ_00078271">
        <obo:RO_0001025 rdf:resource="http://purl.obolibrary.org/obo/GAZ_00078216"/>
        <oboInOwl:hasOBONamespace>GAZ</oboInOwl:hasOBONamespace>
        <oboInOwl:id>GAZ:00078271</oboInOwl:id>
        <rdfs:label>City of Jaffa</rdfs:label>
    </owl:NamedIndividual>
    


    <!-- http://purl.obolibrary.org/obo/GAZ_00078272 -->

    <owl:NamedIndividual rdf:about="http://purl.obolibrary.org/obo/GAZ_00078272">
        <obo:RO_0001025 rdf:resource="http://purl.obolibrary.org/obo/GAZ_00078215"/>
        <obo:IAO_0000115>A populated place. A city in Israel, on the central coastal strip, just south of Tel Aviv, and part of the metropolitan area known as Gush Dan in the Tel Aviv District.</obo:IAO_0000115>
        <oboInOwl:hasOBONamespace>GAZ</oboInOwl:hasOBONamespace>
        <oboInOwl:id>GAZ:00078272</oboInOwl:id>
        <rdfs:label>City of Holon</rdfs:label>
    </owl:NamedIndividual>
    


    <!-- http://purl.obolibrary.org/obo/GAZ_00078273 -->

    <owl:NamedIndividual rdf:about="http://purl.obolibrary.org/obo/GAZ_00078273">
        <obo:RO_0001025 rdf:resource="http://purl.obolibrary.org/obo/GAZ_00078213"/>
        <obo:IAO_0000115>A city located on Israel&apos;s Mediterranean coast, on the central coastal strip, just south of Tel Aviv. Part of the Gush Dan metropolitan area, in the Tel Aviv District, the city is located on the Mediterranean Sea.</obo:IAO_0000115>
        <oboInOwl:hasOBONamespace>GAZ</oboInOwl:hasOBONamespace>
        <oboInOwl:id>GAZ:00078273</oboInOwl:id>
        <rdfs:label>City of Bat Yam</rdfs:label>
    </owl:NamedIndividual>
    


    <!-- http://purl.obolibrary.org/obo/GAZ_00078274 -->

    <owl:NamedIndividual rdf:about="http://purl.obolibrary.org/obo/GAZ_00078274">
        <obo:RO_0001025 rdf:resource="http://purl.obolibrary.org/obo/GAZ_00078213"/>
        <obo:IAO_0000115>A city located on Israel&apos;s central coastal strip in the south of the Sharon region, bordering Tel Aviv to the south and Herzliya and Kibbutz Glil Yam to the north. It is part of the Gush Dan Tel Aviv metropolitan area and is in the Tel Aviv District.</obo:IAO_0000115>
        <oboInOwl:hasOBONamespace>GAZ</oboInOwl:hasOBONamespace>
        <oboInOwl:id>GAZ:00078274</oboInOwl:id>
        <rdfs:label>City of Ramat HaSharon</rdfs:label>
    </owl:NamedIndividual>
    


    <!-- http://purl.obolibrary.org/obo/GAZ_00078275 -->

    <owl:NamedIndividual rdf:about="http://purl.obolibrary.org/obo/GAZ_00078275">
        <obo:RO_0001025 rdf:resource="http://purl.obolibrary.org/obo/GAZ_00078213"/>
        <obo:IAO_0000115>A populated place. A city in Israel. It is located just east of Tel Aviv, and is a part of the metropolitan area known as Gush Dan in the Tel Aviv District.</obo:IAO_0000115>
        <oboInOwl:hasOBONamespace>GAZ</oboInOwl:hasOBONamespace>
        <oboInOwl:id>GAZ:00078275</oboInOwl:id>
        <rdfs:label>City of Giv&apos;atayim</rdfs:label>
    </owl:NamedIndividual>
    


    <!-- http://purl.obolibrary.org/obo/GAZ_00078276 -->

    <owl:NamedIndividual rdf:about="http://purl.obolibrary.org/obo/GAZ_00078276">
        <obo:RO_0001025 rdf:resource="http://purl.obolibrary.org/obo/GAZ_00078213"/>
        <obo:IAO_0000115>A populated place. A city in the Tel Aviv District of Israel. It is located 11 km east of Tel Aviv.</obo:IAO_0000115>
        <oboInOwl:hasOBONamespace>GAZ</oboInOwl:hasOBONamespace>
        <oboInOwl:id>GAZ:00078276</oboInOwl:id>
        <rdfs:label>City of Kiryat Ono</rdfs:label>
    </owl:NamedIndividual>
    


    <!-- http://purl.obolibrary.org/obo/GAZ_00078277 -->

    <owl:NamedIndividual rdf:about="http://purl.obolibrary.org/obo/GAZ_00078277">
        <obo:RO_0001025 rdf:resource="http://purl.obolibrary.org/obo/GAZ_00078214"/>
        <obo:IAO_0000115>A populated place. A city in the Tel Aviv district, Israel, which borders the cities of Tel Aviv, Giv&apos;atayim, Bnei Brak, Kiryat Ono and Givat Shmuel.</obo:IAO_0000115>
        <oboInOwl:hasOBONamespace>GAZ</oboInOwl:hasOBONamespace>
        <oboInOwl:id>GAZ:00078277</oboInOwl:id>
        <rdfs:label>City of Ramat Gan</rdfs:label>
    </owl:NamedIndividual>
    


    <!-- http://purl.obolibrary.org/obo/GAZ_00078278 -->

    <owl:NamedIndividual rdf:about="http://purl.obolibrary.org/obo/GAZ_00078278">
        <obo:RO_0001025 rdf:resource="http://purl.obolibrary.org/obo/GAZ_00078213"/>
        <obo:IAO_0000115>A city located on Israel&apos;s central coastal strip, just north of Tel Aviv. It is part of the Tel Aviv District.</obo:IAO_0000115>
        <oboInOwl:hasOBONamespace>GAZ</oboInOwl:hasOBONamespace>
        <oboInOwl:id>GAZ:00078278</oboInOwl:id>
        <rdfs:label>City of Herzliya</rdfs:label>
    </owl:NamedIndividual>
    


    <!-- http://purl.obolibrary.org/obo/GAZ_00078279 -->

    <owl:NamedIndividual rdf:about="http://purl.obolibrary.org/obo/GAZ_00078279">
        <obo:RO_0001025 rdf:resource="http://purl.obolibrary.org/obo/GAZ_00078213"/>
        <obo:IAO_0000115>A populated place. A city in the Tel Aviv District in Israel.</obo:IAO_0000115>
        <oboInOwl:hasOBONamespace>GAZ</oboInOwl:hasOBONamespace>
        <oboInOwl:id>GAZ:00078279</oboInOwl:id>
        <rdfs:label>City of Or Yehuda</rdfs:label>
    </owl:NamedIndividual>
    


    <!-- http://purl.obolibrary.org/obo/GAZ_00078280 -->

    <owl:NamedIndividual rdf:about="http://purl.obolibrary.org/obo/GAZ_00078280">
        <obo:RO_0001025 rdf:resource="http://purl.obolibrary.org/obo/GAZ_00078213"/>
        <obo:IAO_0000115>A city located on Israel&apos;s central Mediterranean coastal plain, just east of Tel Aviv, in the Dan metropolitan region and Tel Aviv District.</obo:IAO_0000115>
        <oboInOwl:hasOBONamespace>GAZ</oboInOwl:hasOBONamespace>
        <oboInOwl:id>GAZ:00078280</oboInOwl:id>
        <rdfs:label>City of Bnei Brak</rdfs:label>
    </owl:NamedIndividual>
    


    <!-- http://purl.obolibrary.org/obo/GAZ_00078281 -->

    <owl:NamedIndividual rdf:about="http://purl.obolibrary.org/obo/GAZ_00078281">
        <obo:RO_0001025 rdf:resource="http://purl.obolibrary.org/obo/GAZ_00002714"/>
        <obo:IAO_0000115>A Local Council in the Sharon region. It is located east of Netanya and north of Kfar Saba.</obo:IAO_0000115>
        <oboInOwl:hasOBONamespace>GAZ</oboInOwl:hasOBONamespace>
        <oboInOwl:id>GAZ:00078281</oboInOwl:id>
        <rdfs:label>Tel Mond Local Council</rdfs:label>
    </owl:NamedIndividual>
    


    <!-- http://purl.obolibrary.org/obo/GAZ_00078282 -->

    <owl:NamedIndividual rdf:about="http://purl.obolibrary.org/obo/GAZ_00078282">
        <obo:RO_0001025 rdf:resource="http://purl.obolibrary.org/obo/GAZ_00078208"/>
        <oboInOwl:hasOBONamespace>GAZ</oboInOwl:hasOBONamespace>
        <oboInOwl:id>GAZ:00078282</oboInOwl:id>
        <rdfs:label>City of Petah Tiqva</rdfs:label>
    </owl:NamedIndividual>
    


    <!-- http://purl.obolibrary.org/obo/GAZ_00078283 -->

    <owl:NamedIndividual rdf:about="http://purl.obolibrary.org/obo/GAZ_00078283">
        <obo:RO_0001025 rdf:resource="http://purl.obolibrary.org/obo/GAZ_00078211"/>
        <oboInOwl:hasOBONamespace>GAZ</oboInOwl:hasOBONamespace>
        <oboInOwl:id>GAZ:00078283</oboInOwl:id>
        <rdfs:label>City of Rehovot</rdfs:label>
    </owl:NamedIndividual>
    


    <!-- http://purl.obolibrary.org/obo/GAZ_00078284 -->

    <owl:NamedIndividual rdf:about="http://purl.obolibrary.org/obo/GAZ_00078284">
        <obo:RO_0001025 rdf:resource="http://purl.obolibrary.org/obo/GAZ_00002714"/>
        <obo:IAO_0000115>The joint municipality of Yehud and the neighboring community of Neve Monosson in central Israel, created by their municipal merger in 2003. Yehud is a city, while Neve Monosson is a communal settlement.</obo:IAO_0000115>
        <oboInOwl:hasOBONamespace>GAZ</oboInOwl:hasOBONamespace>
        <oboInOwl:id>GAZ:00078284</oboInOwl:id>
        <rdfs:label>City of Yehud-Monosson</rdfs:label>
    </owl:NamedIndividual>
    


    <!-- http://purl.obolibrary.org/obo/GAZ_00078285 -->

    <owl:NamedIndividual rdf:about="http://purl.obolibrary.org/obo/GAZ_00078285">
        <obo:RO_0001025 rdf:resource="http://purl.obolibrary.org/obo/GAZ_00002714"/>
        <obo:IAO_0000115>A city on Israel&apos;s central coastal plain, south of Tel Aviv. It is part of the Gush Dan Greater Tel Aviv metropolitan area.</obo:IAO_0000115>
        <oboInOwl:hasOBONamespace>GAZ</oboInOwl:hasOBONamespace>
        <oboInOwl:id>GAZ:00078285</oboInOwl:id>
        <rdfs:label>City of Rishon LeZion</rdfs:label>
    </owl:NamedIndividual>
    


    <!-- http://purl.obolibrary.org/obo/GAZ_00078286 -->

    <owl:NamedIndividual rdf:about="http://purl.obolibrary.org/obo/GAZ_00078286">
        <obo:RO_0001025 rdf:resource="http://purl.obolibrary.org/obo/GAZ_00002714"/>
        <obo:IAO_0000115>A populated place. A city in the southern Sharon Plain in the Center District of Israel, 19 km north of Tel Aviv.</obo:IAO_0000115>
        <oboInOwl:hasOBONamespace>GAZ</oboInOwl:hasOBONamespace>
        <oboInOwl:id>GAZ:00078286</oboInOwl:id>
        <rdfs:label>City of Ra&apos;annana</rdfs:label>
    </owl:NamedIndividual>
    


    <!-- http://purl.obolibrary.org/obo/GAZ_00078287 -->

    <owl:NamedIndividual rdf:about="http://purl.obolibrary.org/obo/GAZ_00078287">
        <obo:RO_0001025 rdf:resource="http://purl.obolibrary.org/obo/GAZ_00002714"/>
        <obo:IAO_0000115>A populated place. A city in the Center District of Israel in Israel.</obo:IAO_0000115>
        <oboInOwl:hasOBONamespace>GAZ</oboInOwl:hasOBONamespace>
        <oboInOwl:id>GAZ:00078287</oboInOwl:id>
        <rdfs:label>City of Ness Ziona</rdfs:label>
    </owl:NamedIndividual>
    


    <!-- http://purl.obolibrary.org/obo/GAZ_00078288 -->

    <owl:NamedIndividual rdf:about="http://purl.obolibrary.org/obo/GAZ_00078288">
        <obo:RO_0001025 rdf:resource="http://purl.obolibrary.org/obo/GAZ_00002714"/>
        <obo:IAO_0000115>An Israeli Arab city in central Israel.</obo:IAO_0000115>
        <oboInOwl:hasOBONamespace>GAZ</oboInOwl:hasOBONamespace>
        <oboInOwl:id>GAZ:00078288</oboInOwl:id>
        <rdfs:label>City of Tayibe</rdfs:label>
    </owl:NamedIndividual>
    


    <!-- http://purl.obolibrary.org/obo/GAZ_00078289 -->

    <owl:NamedIndividual rdf:about="http://purl.obolibrary.org/obo/GAZ_00078289">
        <obo:RO_0001025 rdf:resource="http://purl.obolibrary.org/obo/GAZ_00002714"/>
        <obo:IAO_0000115>A populated place. A city in the Central District of Israel.</obo:IAO_0000115>
        <oboInOwl:hasOBONamespace>GAZ</oboInOwl:hasOBONamespace>
        <oboInOwl:id>GAZ:00078289</oboInOwl:id>
        <rdfs:label>City of Lod</rdfs:label>
    </owl:NamedIndividual>
    


    <!-- http://purl.obolibrary.org/obo/GAZ_00078290 -->

    <owl:NamedIndividual rdf:about="http://purl.obolibrary.org/obo/GAZ_00078290">
        <obo:RO_0001025 rdf:resource="http://purl.obolibrary.org/obo/GAZ_00002714"/>
        <obo:IAO_0000115>A populated place. A city in the Center District of Israel in Israel.</obo:IAO_0000115>
        <oboInOwl:hasOBONamespace>GAZ</oboInOwl:hasOBONamespace>
        <oboInOwl:id>GAZ:00078290</oboInOwl:id>
        <rdfs:label>City of Rosh HaAyin</rdfs:label>
    </owl:NamedIndividual>
    


    <!-- http://purl.obolibrary.org/obo/GAZ_00078291 -->

    <owl:NamedIndividual rdf:about="http://purl.obolibrary.org/obo/GAZ_00078291">
        <obo:RO_0001025 rdf:resource="http://purl.obolibrary.org/obo/GAZ_00002714"/>
        <obo:IAO_0000115>A populated place. A city in the Center District of Israel. It is the result of the merger of Modi&apos;in and Maccabim-Re&apos;ut in 2003.</obo:IAO_0000115>
        <oboInOwl:hasOBONamespace>GAZ</oboInOwl:hasOBONamespace>
        <oboInOwl:id>GAZ:00078291</oboInOwl:id>
        <rdfs:label>City of Modi&apos;in-Maccabim-Re&apos;ut</rdfs:label>
    </owl:NamedIndividual>
    


    <!-- http://purl.obolibrary.org/obo/GAZ_00078292 -->

    <owl:NamedIndividual rdf:about="http://purl.obolibrary.org/obo/GAZ_00078292">
        <obo:RO_0001025 rdf:resource="http://purl.obolibrary.org/obo/GAZ_00002714"/>
        <obo:IAO_0000115>A populated place. A city in the Center District of Israel.</obo:IAO_0000115>
        <oboInOwl:hasOBONamespace>GAZ</oboInOwl:hasOBONamespace>
        <oboInOwl:id>GAZ:00078292</oboInOwl:id>
        <rdfs:label>City of Qalansawe</rdfs:label>
    </owl:NamedIndividual>
    


    <!-- http://purl.obolibrary.org/obo/GAZ_00078293 -->

    <owl:NamedIndividual rdf:about="http://purl.obolibrary.org/obo/GAZ_00078293">
        <obo:RO_0001025 rdf:resource="http://purl.obolibrary.org/obo/GAZ_00002714"/>
        <obo:IAO_0000115>A hill-top Israeli Arab city located about twenty km east of Tel Aviv, near the Green Line separating Israel and the West Bank, on the southern portion of the &quot;Little Triangle&quot; of Arab-Israeli towns and villages.</obo:IAO_0000115>
        <oboInOwl:hasOBONamespace>GAZ</oboInOwl:hasOBONamespace>
        <oboInOwl:id>GAZ:00078293</oboInOwl:id>
        <rdfs:label>City of Kafr Qasim</rdfs:label>
    </owl:NamedIndividual>
    


    <!-- http://purl.obolibrary.org/obo/GAZ_00078294 -->

    <owl:NamedIndividual rdf:about="http://purl.obolibrary.org/obo/GAZ_00078294">
        <obo:RO_0001025 rdf:resource="http://purl.obolibrary.org/obo/GAZ_00002714"/>
        <obo:IAO_0000115>A populated place. A city in the Center District of Israel.</obo:IAO_0000115>
        <oboInOwl:hasOBONamespace>GAZ</oboInOwl:hasOBONamespace>
        <oboInOwl:id>GAZ:00078294</oboInOwl:id>
        <rdfs:label>City of Yavne</rdfs:label>
    </owl:NamedIndividual>
    


    <!-- http://purl.obolibrary.org/obo/GAZ_00078295 -->

    <owl:NamedIndividual rdf:about="http://purl.obolibrary.org/obo/GAZ_00078295">
        <obo:RO_0001025 rdf:resource="http://purl.obolibrary.org/obo/GAZ_00002714"/>
        <obo:IAO_0000115>A populated place. A city in the Center District of Israel in Israel.</obo:IAO_0000115>
        <oboInOwl:hasOBONamespace>GAZ</oboInOwl:hasOBONamespace>
        <oboInOwl:id>GAZ:00078295</oboInOwl:id>
        <rdfs:label>City of Tira</rdfs:label>
    </owl:NamedIndividual>
    


    <!-- http://purl.obolibrary.org/obo/GAZ_00078296 -->

    <owl:NamedIndividual rdf:about="http://purl.obolibrary.org/obo/GAZ_00078296">
        <obo:RO_0001025 rdf:resource="http://purl.obolibrary.org/obo/GAZ_00002714"/>
        <obo:IAO_0000115>A populated place. A city in central Israel.</obo:IAO_0000115>
        <oboInOwl:hasOBONamespace>GAZ</oboInOwl:hasOBONamespace>
        <oboInOwl:id>GAZ:00078296</oboInOwl:id>
        <rdfs:label>City of Ramla</rdfs:label>
    </owl:NamedIndividual>
    


    <!-- http://purl.obolibrary.org/obo/GAZ_00078297 -->

    <owl:NamedIndividual rdf:about="http://purl.obolibrary.org/obo/GAZ_00078297">
        <obo:RO_0001025 rdf:resource="http://purl.obolibrary.org/obo/GAZ_00002714"/>
        <obo:IAO_0000115>A populated place. A city in the Center District of Israel. Officially declared a city in 1990, Hod HaSharon was created from the union in 1964 of four neighboring small towns: Magdiel, Ramatayim, Kfar Hadar, and Ramat Hadar.</obo:IAO_0000115>
        <oboInOwl:hasOBONamespace>GAZ</oboInOwl:hasOBONamespace>
        <oboInOwl:id>GAZ:00078297</oboInOwl:id>
        <rdfs:label>City of Hod Hasharon</rdfs:label>
    </owl:NamedIndividual>
    


    <!-- http://purl.obolibrary.org/obo/GAZ_00078298 -->

    <owl:NamedIndividual rdf:about="http://purl.obolibrary.org/obo/GAZ_00078298">
        <obo:RO_0001025 rdf:resource="http://purl.obolibrary.org/obo/GAZ_00002714"/>
        <obo:IAO_0000115>A populated place. A city in the Centre District of Israel and is the capital of the Sharon plain. It is located between the &apos;Poleg&apos; stream and Wingate Institute in the south and the &apos;Avichail&apos; stream in the north.</obo:IAO_0000115>
        <oboInOwl:hasOBONamespace>GAZ</oboInOwl:hasOBONamespace>
        <oboInOwl:id>GAZ:00078298</oboInOwl:id>
        <rdfs:label>City of Netanya</rdfs:label>
    </owl:NamedIndividual>
    


    <!-- http://purl.obolibrary.org/obo/GAZ_00078299 -->

    <owl:NamedIndividual rdf:about="http://purl.obolibrary.org/obo/GAZ_00078299">
        <obo:RO_0001025 rdf:resource="http://purl.obolibrary.org/obo/GAZ_00002714"/>
        <obo:IAO_0000115>A populated place. A city in the Sharon region, of the Center District of Israel.</obo:IAO_0000115>
        <oboInOwl:hasOBONamespace>GAZ</oboInOwl:hasOBONamespace>
        <oboInOwl:id>GAZ:00078299</oboInOwl:id>
        <rdfs:label>City of Kfar Saba</rdfs:label>
    </owl:NamedIndividual>
    


    <!-- http://purl.obolibrary.org/obo/GAZ_00078300 -->

    <owl:NamedIndividual rdf:about="http://purl.obolibrary.org/obo/GAZ_00078300">
        <obo:RO_0001025 rdf:resource="http://purl.obolibrary.org/obo/GAZ_00002714"/>
        <obo:IAO_0000115>A Local Council in the Center District of Israel. It is located between the cities of Rehovot to the north, Ashdod to the west.</obo:IAO_0000115>
        <oboInOwl:hasOBONamespace>GAZ</oboInOwl:hasOBONamespace>
        <oboInOwl:id>GAZ:00078300</oboInOwl:id>
        <rdfs:label>Gedera Local Council</rdfs:label>
    </owl:NamedIndividual>
    


    <!-- http://purl.obolibrary.org/obo/GAZ_00078301 -->

    <owl:NamedIndividual rdf:about="http://purl.obolibrary.org/obo/GAZ_00078301">
        <obo:RO_0001025 rdf:resource="http://purl.obolibrary.org/obo/GAZ_00002714"/>
        <obo:IAO_0000115>A Local Council in the Center District of Israel. Located about 25 km east of Tel Aviv on Route 444 between Rosh HaAyin and Shoham, it also lies just west of the Green Line.</obo:IAO_0000115>
        <oboInOwl:hasOBONamespace>GAZ</oboInOwl:hasOBONamespace>
        <oboInOwl:id>GAZ:00078301</oboInOwl:id>
        <rdfs:label>El&apos;ad Local Council</rdfs:label>
    </owl:NamedIndividual>
    


    <!-- http://purl.obolibrary.org/obo/GAZ_00078302 -->

    <owl:NamedIndividual rdf:about="http://purl.obolibrary.org/obo/GAZ_00078302">
        <obo:RO_0001025 rdf:resource="http://purl.obolibrary.org/obo/GAZ_00002714"/>
        <obo:IAO_0000115>A Local Council in the Center District of Israel.</obo:IAO_0000115>
        <oboInOwl:hasOBONamespace>GAZ</oboInOwl:hasOBONamespace>
        <oboInOwl:id>GAZ:00078302</oboInOwl:id>
        <rdfs:label>Elyakhin Local Council</rdfs:label>
    </owl:NamedIndividual>
    


    <!-- http://purl.obolibrary.org/obo/GAZ_00078303 -->

    <owl:NamedIndividual rdf:about="http://purl.obolibrary.org/obo/GAZ_00078303">
        <obo:RO_0001025 rdf:resource="http://purl.obolibrary.org/obo/GAZ_00002714"/>
        <obo:IAO_0000115>A Local Council in Israel surrounded by the major cities Ramat Gan, Bnei Brak, Kiryat Ono and Petah Tikva. It is located in Gush Dan.</obo:IAO_0000115>
        <oboInOwl:hasOBONamespace>GAZ</oboInOwl:hasOBONamespace>
        <oboInOwl:id>GAZ:00078303</oboInOwl:id>
        <rdfs:label>Giv&apos;at Shmuel Local Council</rdfs:label>
    </owl:NamedIndividual>
    


    <!-- http://purl.obolibrary.org/obo/GAZ_00078304 -->

    <owl:NamedIndividual rdf:about="http://purl.obolibrary.org/obo/GAZ_00078304">
        <obo:RO_0001025 rdf:resource="http://purl.obolibrary.org/obo/GAZ_00002714"/>
        <obo:IAO_0000115>A Local Council in the Center District of Israel, located near the city of Ashdod.</obo:IAO_0000115>
        <oboInOwl:hasOBONamespace>GAZ</oboInOwl:hasOBONamespace>
        <oboInOwl:id>GAZ:00078304</oboInOwl:id>
        <rdfs:label>Gan Yavne Local Council</rdfs:label>
    </owl:NamedIndividual>
    


    <!-- http://purl.obolibrary.org/obo/GAZ_00078305 -->

    <owl:NamedIndividual rdf:about="http://purl.obolibrary.org/obo/GAZ_00078305">
        <obo:RO_0001025 rdf:resource="http://purl.obolibrary.org/obo/GAZ_00002714"/>
        <obo:IAO_0000115>A Local Council in the Center District of Israel, about ten km from Ashdod and bordering Gedera.</obo:IAO_0000115>
        <oboInOwl:hasOBONamespace>GAZ</oboInOwl:hasOBONamespace>
        <oboInOwl:id>GAZ:00078305</oboInOwl:id>
        <rdfs:label>Bnei Aish Local Council</rdfs:label>
    </owl:NamedIndividual>
    


    <!-- http://purl.obolibrary.org/obo/GAZ_00078306 -->

    <owl:NamedIndividual rdf:about="http://purl.obolibrary.org/obo/GAZ_00078306">
        <obo:RO_0001025 rdf:resource="http://purl.obolibrary.org/obo/GAZ_00002714"/>
        <obo:IAO_0000115>A Local Council in the center of Israel.</obo:IAO_0000115>
        <oboInOwl:hasOBONamespace>GAZ</oboInOwl:hasOBONamespace>
        <oboInOwl:id>GAZ:00078306</oboInOwl:id>
        <rdfs:label>Mazkeret Batya Local Council</rdfs:label>
    </owl:NamedIndividual>
    


    <!-- http://purl.obolibrary.org/obo/GAZ_00078307 -->

    <owl:NamedIndividual rdf:about="http://purl.obolibrary.org/obo/GAZ_00078307">
        <obo:RO_0001025 rdf:resource="http://purl.obolibrary.org/obo/GAZ_00002714"/>
        <obo:IAO_0000115>A local council in the Center District of Israel.</obo:IAO_0000115>
        <oboInOwl:hasOBONamespace>GAZ</oboInOwl:hasOBONamespace>
        <oboInOwl:id>GAZ:00078307</oboInOwl:id>
        <rdfs:label>Be&apos;er Ya&apos;aqov Local Council</rdfs:label>
    </owl:NamedIndividual>
    


    <!-- http://purl.obolibrary.org/obo/GAZ_00078308 -->

    <owl:NamedIndividual rdf:about="http://purl.obolibrary.org/obo/GAZ_00078308">
        <obo:RO_0001025 rdf:resource="http://purl.obolibrary.org/obo/GAZ_00002714"/>
        <obo:IAO_0000115>A Local Council located in the central Sharon region of Israel, near the city of Netanya.</obo:IAO_0000115>
        <oboInOwl:hasOBONamespace>GAZ</oboInOwl:hasOBONamespace>
        <oboInOwl:id>GAZ:00078308</oboInOwl:id>
        <rdfs:label>Even Yehuda Local Council</rdfs:label>
    </owl:NamedIndividual>
    


    <!-- http://purl.obolibrary.org/obo/GAZ_00078309 -->

    <owl:NamedIndividual rdf:about="http://purl.obolibrary.org/obo/GAZ_00078309">
        <obo:RO_0001025 rdf:resource="http://purl.obolibrary.org/obo/GAZ_00002714"/>
        <obo:IAO_0000115>A Local Council in the Center District of Israel, bordering Rishon LeZion.</obo:IAO_0000115>
        <oboInOwl:hasOBONamespace>GAZ</oboInOwl:hasOBONamespace>
        <oboInOwl:id>GAZ:00078309</oboInOwl:id>
        <rdfs:label>Beit Dagan Local Council</rdfs:label>
    </owl:NamedIndividual>
    


    <!-- http://purl.obolibrary.org/obo/GAZ_00078310 -->

    <owl:NamedIndividual rdf:about="http://purl.obolibrary.org/obo/GAZ_00078310">
        <obo:RO_0001025 rdf:resource="http://purl.obolibrary.org/obo/GAZ_00002714"/>
        <obo:IAO_0000115>A Local Council located on the coastal plain in the Central Region of Israel.</obo:IAO_0000115>
        <oboInOwl:hasOBONamespace>GAZ</oboInOwl:hasOBONamespace>
        <oboInOwl:id>GAZ:00078310</oboInOwl:id>
        <rdfs:label>Kiryat Ekron Local Council</rdfs:label>
    </owl:NamedIndividual>
    


    <!-- http://purl.obolibrary.org/obo/GAZ_00078311 -->

    <owl:NamedIndividual rdf:about="http://purl.obolibrary.org/obo/GAZ_00078311">
        <obo:RO_0001025 rdf:resource="http://purl.obolibrary.org/obo/GAZ_00002714"/>
        <obo:IAO_0000115>A local council in the Center District of Israel, located next to Hod HaSharon and Kfar Saba.</obo:IAO_0000115>
        <oboInOwl:hasOBONamespace>GAZ</oboInOwl:hasOBONamespace>
        <oboInOwl:id>GAZ:00078311</oboInOwl:id>
        <rdfs:label>Jaljulia Local Council</rdfs:label>
    </owl:NamedIndividual>
    


    <!-- http://purl.obolibrary.org/obo/GAZ_00078312 -->

    <owl:NamedIndividual rdf:about="http://purl.obolibrary.org/obo/GAZ_00078312">
        <obo:RO_0001025 rdf:resource="http://purl.obolibrary.org/obo/GAZ_00002714"/>
        <obo:IAO_0000115>A Local Council in the Center District of Israel.</obo:IAO_0000115>
        <oboInOwl:hasOBONamespace>GAZ</oboInOwl:hasOBONamespace>
        <oboInOwl:id>GAZ:00078312</oboInOwl:id>
        <rdfs:label>Ramot Hashavim Local Council</rdfs:label>
    </owl:NamedIndividual>
    


    <!-- http://purl.obolibrary.org/obo/GAZ_00078313 -->

    <owl:NamedIndividual rdf:about="http://purl.obolibrary.org/obo/GAZ_00078313">
        <obo:RO_0001025 rdf:resource="http://purl.obolibrary.org/obo/GAZ_00002714"/>
        <obo:IAO_0000115>A Local Council in the Center District of Israel.</obo:IAO_0000115>
        <oboInOwl:hasOBONamespace>GAZ</oboInOwl:hasOBONamespace>
        <oboInOwl:id>GAZ:00078313</oboInOwl:id>
        <rdfs:label>Pardesiya Local Council</rdfs:label>
    </owl:NamedIndividual>
    


    <!-- http://purl.obolibrary.org/obo/GAZ_00078314 -->

    <owl:NamedIndividual rdf:about="http://purl.obolibrary.org/obo/GAZ_00078314">
        <obo:RO_0001025 rdf:resource="http://purl.obolibrary.org/obo/GAZ_00002714"/>
        <obo:IAO_0000115>A Local Council in the Sharon Subdistrict in the Center District of Israel. It is about 11 km east of the Mediterranean sea shore city of Netanya, and about 15km west of the border with Palestinian Authority-held Tulkarm.</obo:IAO_0000115>
        <oboInOwl:hasOBONamespace>GAZ</oboInOwl:hasOBONamespace>
        <oboInOwl:id>GAZ:00078314</oboInOwl:id>
        <rdfs:label>Kfar Yona Local Council</rdfs:label>
    </owl:NamedIndividual>
    


    <!-- http://purl.obolibrary.org/obo/GAZ_00078315 -->

    <owl:NamedIndividual rdf:about="http://purl.obolibrary.org/obo/GAZ_00078315">
        <obo:RO_0001025 rdf:resource="http://purl.obolibrary.org/obo/GAZ_00002714"/>
        <obo:IAO_0000115>A local council in Israel, located in the midst of the Kiryat Ono, Petah Tikva and Or Yehuda triangle.</obo:IAO_0000115>
        <oboInOwl:hasOBONamespace>GAZ</oboInOwl:hasOBONamespace>
        <oboInOwl:id>GAZ:00078315</oboInOwl:id>
        <rdfs:label>Savyon Local Council</rdfs:label>
    </owl:NamedIndividual>
    


    <!-- http://purl.obolibrary.org/obo/GAZ_00078316 -->

    <owl:NamedIndividual rdf:about="http://purl.obolibrary.org/obo/GAZ_00078316">
        <obo:RO_0001025 rdf:resource="http://purl.obolibrary.org/obo/GAZ_00002714"/>
        <obo:IAO_0000115>A local council in Israel, bordering Kiryat Ono on the west, Petah Tikva on the north, Gat Rimon on the east and Savyon on the south.</obo:IAO_0000115>
        <oboInOwl:hasOBONamespace>GAZ</oboInOwl:hasOBONamespace>
        <oboInOwl:id>GAZ:00078316</oboInOwl:id>
        <rdfs:label>Ganei Tikva Local Council</rdfs:label>
    </owl:NamedIndividual>
    


    <!-- http://purl.obolibrary.org/obo/GAZ_00078317 -->

    <owl:NamedIndividual rdf:about="http://purl.obolibrary.org/obo/GAZ_00078317">
        <obo:RO_0001025 rdf:resource="http://purl.obolibrary.org/obo/GAZ_00002714"/>
        <obo:IAO_0000115>An Israeli-Arab local council in Israel&apos;s Center District. The small town, located near the Green Line, is often considered a part of the Little Triangle along with Kafr Qasim and Jaljulia.</obo:IAO_0000115>
        <oboInOwl:hasOBONamespace>GAZ</oboInOwl:hasOBONamespace>
        <oboInOwl:id>GAZ:00078317</oboInOwl:id>
        <rdfs:label>Kfar Bara Local Council</rdfs:label>
    </owl:NamedIndividual>
    


    <!-- http://purl.obolibrary.org/obo/GAZ_00078318 -->

    <owl:NamedIndividual rdf:about="http://purl.obolibrary.org/obo/GAZ_00078318">
        <obo:RO_0001025 rdf:resource="http://purl.obolibrary.org/obo/GAZ_00002714"/>
        <obo:IAO_0000115>A Local Council in the Center District of Israel.</obo:IAO_0000115>
        <oboInOwl:hasOBONamespace>GAZ</oboInOwl:hasOBONamespace>
        <oboInOwl:id>GAZ:00078318</oboInOwl:id>
        <rdfs:label>Shoham Local Council</rdfs:label>
    </owl:NamedIndividual>
    


    <!-- http://purl.obolibrary.org/obo/GAZ_00078319 -->

    <owl:NamedIndividual rdf:about="http://purl.obolibrary.org/obo/GAZ_00078319">
        <obo:RO_0001025 rdf:resource="http://purl.obolibrary.org/obo/GAZ_00002714"/>
        <obo:IAO_0000115>A Local Council in the Center District of Israel.</obo:IAO_0000115>
        <oboInOwl:hasOBONamespace>GAZ</oboInOwl:hasOBONamespace>
        <oboInOwl:id>GAZ:00078319</oboInOwl:id>
        <rdfs:label>Zemer Local Council</rdfs:label>
    </owl:NamedIndividual>
    


    <!-- http://purl.obolibrary.org/obo/GAZ_00078320 -->

    <owl:NamedIndividual rdf:about="http://purl.obolibrary.org/obo/GAZ_00078320">
        <obo:RO_0001025 rdf:resource="http://purl.obolibrary.org/obo/GAZ_00002714"/>
        <obo:IAO_0000115>A local council in the Center District of Israel. It is the result of the 2003 union of the Tzoran and Kadima councils.</obo:IAO_0000115>
        <oboInOwl:hasOBONamespace>GAZ</oboInOwl:hasOBONamespace>
        <oboInOwl:id>GAZ:00078320</oboInOwl:id>
        <rdfs:label>Tzoran-Kadima Local Council</rdfs:label>
    </owl:NamedIndividual>
    


    <!-- http://purl.obolibrary.org/obo/GAZ_00078321 -->

    <owl:NamedIndividual rdf:about="http://purl.obolibrary.org/obo/GAZ_00078321">
        <obo:RO_0001025 rdf:resource="http://purl.obolibrary.org/obo/GAZ_00002714"/>
        <obo:IAO_0000115>A Local Council in the Center District of Israel. The municipality merged with the neighboring town of Tzur Yigal in 2003-11.</obo:IAO_0000115>
        <oboInOwl:hasOBONamespace>GAZ</oboInOwl:hasOBONamespace>
        <oboInOwl:id>GAZ:00078321</oboInOwl:id>
        <rdfs:label>Kokhav Yair Local Council</rdfs:label>
    </owl:NamedIndividual>
    


    <!-- http://purl.obolibrary.org/obo/GAZ_00078322 -->

    <owl:NamedIndividual rdf:about="http://purl.obolibrary.org/obo/GAZ_00078322">
        <obo:RO_0001025 rdf:resource="http://purl.obolibrary.org/obo/GAZ_00078201"/>
        <obo:IAO_0000115>The largest city in Northern Israel, and the third-largest city in the country. The city is a seaport located on Israel&apos;s Mediterranean coastline in the Bay of Haifa.</obo:IAO_0000115>
        <oboInOwl:hasOBONamespace>GAZ</oboInOwl:hasOBONamespace>
        <oboInOwl:id>GAZ:00078322</oboInOwl:id>
        <rdfs:label>City of Haifa</rdfs:label>
    </owl:NamedIndividual>
    


    <!-- http://purl.obolibrary.org/obo/GAZ_00078323 -->

    <owl:NamedIndividual rdf:about="http://purl.obolibrary.org/obo/GAZ_00078323">
        <obo:RO_0001025 rdf:resource="http://purl.obolibrary.org/obo/GAZ_00078203"/>
        <obo:IAO_0000115>A city located in the Haifa District of Israel approximately half-way between the major cities of Tel Aviv and Haifa.</obo:IAO_0000115>
        <oboInOwl:hasOBONamespace>GAZ</oboInOwl:hasOBONamespace>
        <oboInOwl:id>GAZ:00078323</oboInOwl:id>
        <rdfs:label>City of Hadera</rdfs:label>
    </owl:NamedIndividual>
    


    <!-- http://purl.obolibrary.org/obo/GAZ_00078324 -->

    <owl:NamedIndividual rdf:about="http://purl.obolibrary.org/obo/GAZ_00078324">
        <obo:RO_0001025 rdf:resource="http://purl.obolibrary.org/obo/GAZ_00078176"/>
        <obo:IAO_0000115>A regional council in the Judean Mountains in Israel.</obo:IAO_0000115>
        <oboInOwl:hasOBONamespace>GAZ</oboInOwl:hasOBONamespace>
        <oboInOwl:id>GAZ:00078324</oboInOwl:id>
        <rdfs:label>Matte Yehuda Regional Council</rdfs:label>
    </owl:NamedIndividual>
    


    <!-- http://purl.obolibrary.org/obo/GAZ_00078325 -->

    <owl:NamedIndividual rdf:about="http://purl.obolibrary.org/obo/GAZ_00078325">
        <obo:RO_0001025 rdf:resource="http://purl.obolibrary.org/obo/GAZ_00002711"/>
        <obo:IAO_0000115>A populated place. A city in the Haifa District in Israel.</obo:IAO_0000115>
        <oboInOwl:hasOBONamespace>GAZ</oboInOwl:hasOBONamespace>
        <oboInOwl:id>GAZ:00078325</oboInOwl:id>
        <rdfs:label>City of Tirat Carmel</rdfs:label>
    </owl:NamedIndividual>
    


    <!-- http://purl.obolibrary.org/obo/GAZ_00078326 -->

    <owl:NamedIndividual rdf:about="http://purl.obolibrary.org/obo/GAZ_00078326">
        <obo:RO_0001025 rdf:resource="http://purl.obolibrary.org/obo/GAZ_00002711"/>
        <obo:IAO_0000115>A Local Council in the Haifa District of Israel. It is located between Kiryat Tiv&apos;on, Kiryat Ata and Nesher, next to roads 70, 75 and 762.</obo:IAO_0000115>
        <oboInOwl:hasOBONamespace>GAZ</oboInOwl:hasOBONamespace>
        <oboInOwl:id>GAZ:00078326</oboInOwl:id>
        <rdfs:label>Rekhasim Local Council</rdfs:label>
    </owl:NamedIndividual>
    


    <!-- http://purl.obolibrary.org/obo/GAZ_00078327 -->

    <owl:NamedIndividual rdf:about="http://purl.obolibrary.org/obo/GAZ_00078327">
        <obo:RO_0001025 rdf:resource="http://purl.obolibrary.org/obo/GAZ_00002711"/>
        <obo:IAO_0000115>An Israeli Arab local council in the Wadi Ara region in the Haifa District. It is located south of Umm al-Fahm just northwest of the Green Line and is part of the triangle.</obo:IAO_0000115>
        <oboInOwl:hasOBONamespace>GAZ</oboInOwl:hasOBONamespace>
        <oboInOwl:id>GAZ:00078327</oboInOwl:id>
        <rdfs:label>Ar&apos;ara Local Council</rdfs:label>
    </owl:NamedIndividual>
    


    <!-- http://purl.obolibrary.org/obo/GAZ_00078328 -->

    <owl:NamedIndividual rdf:about="http://purl.obolibrary.org/obo/GAZ_00078328">
        <obo:RO_0001025 rdf:resource="http://purl.obolibrary.org/obo/GAZ_00002711"/>
        <obo:IAO_0000115>A populated place. A city in the Haifa District of Israel, located around Mount Carmel.</obo:IAO_0000115>
        <oboInOwl:hasOBONamespace>GAZ</oboInOwl:hasOBONamespace>
        <oboInOwl:id>GAZ:00078328</oboInOwl:id>
        <rdfs:label>Carmel City</rdfs:label>
    </owl:NamedIndividual>
    


    <!-- http://purl.obolibrary.org/obo/GAZ_00078329 -->

    <owl:NamedIndividual rdf:about="http://purl.obolibrary.org/obo/GAZ_00078329">
        <obo:RO_0001025 rdf:resource="http://purl.obolibrary.org/obo/GAZ_00002711"/>
        <obo:IAO_0000115>An Local Council in the Haifa District of Israel.</obo:IAO_0000115>
        <oboInOwl:hasOBONamespace>GAZ</oboInOwl:hasOBONamespace>
        <oboInOwl:id>GAZ:00078329</oboInOwl:id>
        <rdfs:label>Pardes Hanna-Karkur Local Council</rdfs:label>
    </owl:NamedIndividual>
    


    <!-- http://purl.obolibrary.org/obo/GAZ_00078330 -->

    <owl:NamedIndividual rdf:about="http://purl.obolibrary.org/obo/GAZ_00078330">
        <obo:RO_0001025 rdf:resource="http://purl.obolibrary.org/obo/GAZ_00002711"/>
        <obo:IAO_0000115>An Israeli-Arab local council in Israel&apos;s Haifa District and is a part of the Wadi Ara region adjacent to the Triangle. The town consists of the five Arab villages of Baiada, Musmus, Salim, Musheirifa and Zalafa.</obo:IAO_0000115>
        <oboInOwl:hasOBONamespace>GAZ</oboInOwl:hasOBONamespace>
        <oboInOwl:id>GAZ:00078330</oboInOwl:id>
        <rdfs:label>Ma&apos;ale Iron Local Council</rdfs:label>
    </owl:NamedIndividual>
    


    <!-- http://purl.obolibrary.org/obo/GAZ_00078331 -->

    <owl:NamedIndividual rdf:about="http://purl.obolibrary.org/obo/GAZ_00078331">
        <obo:RO_0001025 rdf:resource="http://purl.obolibrary.org/obo/GAZ_00002711"/>
        <obo:IAO_0000115>A Local Council in the Haifa District of Israel, in the hills between the Zvulun and Jezreel valleys. Kiryat Tiv&apos;on is situated 15 km southeast of Haifa, on the main road to Nazareth.</obo:IAO_0000115>
        <oboInOwl:hasOBONamespace>GAZ</oboInOwl:hasOBONamespace>
        <oboInOwl:id>GAZ:00078331</oboInOwl:id>
        <rdfs:label>Kiryat Tivon Local Council</rdfs:label>
    </owl:NamedIndividual>
    


    <!-- http://purl.obolibrary.org/obo/GAZ_00078332 -->

    <owl:NamedIndividual rdf:about="http://purl.obolibrary.org/obo/GAZ_00078332">
        <obo:RO_0001025 rdf:resource="http://purl.obolibrary.org/obo/GAZ_00002711"/>
        <obo:IAO_0000115>A populated place. A city in the Haifa Bay district of Israel, 12 km north of Haifa. One of a group of Haifa suburbs known as the Krayot, it is located on the Mediterranean coast, between Kiryat Haim and the Tzur Shalom industrial area, east of Kiryat Motzkin.</obo:IAO_0000115>
        <oboInOwl:hasOBONamespace>GAZ</oboInOwl:hasOBONamespace>
        <oboInOwl:id>GAZ:00078332</oboInOwl:id>
        <rdfs:label>City of Kiryat Yam</rdfs:label>
    </owl:NamedIndividual>
    


    <!-- http://purl.obolibrary.org/obo/GAZ_00078333 -->

    <owl:NamedIndividual rdf:about="http://purl.obolibrary.org/obo/GAZ_00078333">
        <obo:RO_0001025 rdf:resource="http://purl.obolibrary.org/obo/GAZ_00002711"/>
        <obo:IAO_0000115>An Israeli-Arab local council located in the Wadi Ara area of the Haifa District. The local council was formed in 1995 through the consolidation of the villages of Barta&apos;a West, Ein as-Sahala, and Muawiya.</obo:IAO_0000115>
        <oboInOwl:hasOBONamespace>GAZ</oboInOwl:hasOBONamespace>
        <oboInOwl:id>GAZ:00078333</oboInOwl:id>
        <rdfs:label>Basma Local Council</rdfs:label>
    </owl:NamedIndividual>
    


    <!-- http://purl.obolibrary.org/obo/GAZ_00078334 -->

    <owl:NamedIndividual rdf:about="http://purl.obolibrary.org/obo/GAZ_00078334">
        <obo:RO_0001025 rdf:resource="http://purl.obolibrary.org/obo/GAZ_00002711"/>
        <obo:IAO_0000115>An Israeli Arab local council in the Haifa District.</obo:IAO_0000115>
        <oboInOwl:hasOBONamespace>GAZ</oboInOwl:hasOBONamespace>
        <oboInOwl:id>GAZ:00078334</oboInOwl:id>
        <rdfs:label>Fureidis Local Council</rdfs:label>
    </owl:NamedIndividual>
    


    <!-- http://purl.obolibrary.org/obo/GAZ_00078335 -->

    <owl:NamedIndividual rdf:about="http://purl.obolibrary.org/obo/GAZ_00078335">
        <obo:RO_0001025 rdf:resource="http://purl.obolibrary.org/obo/GAZ_00002711"/>
        <obo:IAO_0000115>An Israeli Arab local council on Israel&apos;s northern Mediterranean coastal plain. Located just north of Caesarea within the Haifa District, it achieved local council status in 1963.</obo:IAO_0000115>
        <oboInOwl:hasOBONamespace>GAZ</oboInOwl:hasOBONamespace>
        <oboInOwl:id>GAZ:00078335</oboInOwl:id>
        <rdfs:label>Jisr az-Zarqa Local Council</rdfs:label>
    </owl:NamedIndividual>
    


    <!-- http://purl.obolibrary.org/obo/GAZ_00078336 -->

    <owl:NamedIndividual rdf:about="http://purl.obolibrary.org/obo/GAZ_00078336">
        <obo:RO_0001025 rdf:resource="http://purl.obolibrary.org/obo/GAZ_00002711"/>
        <obo:IAO_0000115>A Local Council in Israel, 35 km south of Haifa, and part of the Haifa District. It is located at the southern end of the Carmel mountain range overlooking the Mediterranean Sea, near the coastal highway (Highway 2).</obo:IAO_0000115>
        <oboInOwl:hasOBONamespace>GAZ</oboInOwl:hasOBONamespace>
        <oboInOwl:id>GAZ:00078336</oboInOwl:id>
        <rdfs:label>Zikhron Ya&apos;aqov Local Council</rdfs:label>
    </owl:NamedIndividual>
    


    <!-- http://purl.obolibrary.org/obo/GAZ_00078337 -->

    <owl:NamedIndividual rdf:about="http://purl.obolibrary.org/obo/GAZ_00078337">
        <obo:RO_0001025 rdf:resource="http://purl.obolibrary.org/obo/GAZ_00002711"/>
        <obo:IAO_0000115>An Israeli-Arab local council located in Israel&apos;s Haifa District 22 mi southeast of the city of Haifa. It is considered part of the triangle and the Wadi Ara region northwest of the Green Line.</obo:IAO_0000115>
        <oboInOwl:hasOBONamespace>GAZ</oboInOwl:hasOBONamespace>
        <oboInOwl:id>GAZ:00078337</oboInOwl:id>
        <rdfs:label>Kafr Qara Local Council</rdfs:label>
    </owl:NamedIndividual>
    


    <!-- http://purl.obolibrary.org/obo/GAZ_00078338 -->

    <owl:NamedIndividual rdf:about="http://purl.obolibrary.org/obo/GAZ_00078338">
        <obo:RO_0001025 rdf:resource="http://purl.obolibrary.org/obo/GAZ_00002711"/>
        <obo:IAO_0000115>A Local Council in the Haifa District of Israel. It is the result of the 2003 merger between the two local councils of Binyamina and Giv&apos;at Ada.</obo:IAO_0000115>
        <oboInOwl:hasOBONamespace>GAZ</oboInOwl:hasOBONamespace>
        <oboInOwl:id>GAZ:00078338</oboInOwl:id>
        <rdfs:label>Binyamina-Giv&apos;at Ada Local Council</rdfs:label>
    </owl:NamedIndividual>
    


    <!-- http://purl.obolibrary.org/obo/GAZ_00078339 -->

    <owl:NamedIndividual rdf:about="http://purl.obolibrary.org/obo/GAZ_00078339">
        <obo:RO_0001025 rdf:resource="http://purl.obolibrary.org/obo/GAZ_00002711"/>
        <obo:IAO_0000115>A populated place. A city in the Haifa District in Israel.</obo:IAO_0000115>
        <oboInOwl:hasOBONamespace>GAZ</oboInOwl:hasOBONamespace>
        <oboInOwl:id>GAZ:00078339</oboInOwl:id>
        <rdfs:label>City of Kiryat Bialik</rdfs:label>
    </owl:NamedIndividual>
    


    <!-- http://purl.obolibrary.org/obo/GAZ_00078340 -->

    <owl:NamedIndividual rdf:about="http://purl.obolibrary.org/obo/GAZ_00078340">
        <obo:RO_0001025 rdf:resource="http://purl.obolibrary.org/obo/GAZ_00002711"/>
        <obo:IAO_0000115>An Israeli-Arab city in the Haifa District of Israel established in 2003 through a merger of Baqa al-Gharbiyye and Jatt.</obo:IAO_0000115>
        <oboInOwl:hasOBONamespace>GAZ</oboInOwl:hasOBONamespace>
        <oboInOwl:id>GAZ:00078340</oboInOwl:id>
        <rdfs:label>City of Baqa-Jatt</rdfs:label>
    </owl:NamedIndividual>
    


    <!-- http://purl.obolibrary.org/obo/GAZ_00078341 -->

    <owl:NamedIndividual rdf:about="http://purl.obolibrary.org/obo/GAZ_00078341">
        <obo:RO_0001025 rdf:resource="http://purl.obolibrary.org/obo/GAZ_00002711"/>
        <obo:IAO_0000115>A populated place. A city in the Haifa District in Israel.</obo:IAO_0000115>
        <oboInOwl:hasOBONamespace>GAZ</oboInOwl:hasOBONamespace>
        <oboInOwl:id>GAZ:00078341</oboInOwl:id>
        <rdfs:label>City of Kiryat Motzkin</rdfs:label>
    </owl:NamedIndividual>
    


    <!-- http://purl.obolibrary.org/obo/GAZ_00078342 -->

    <owl:NamedIndividual rdf:about="http://purl.obolibrary.org/obo/GAZ_00078342">
        <obo:RO_0001025 rdf:resource="http://purl.obolibrary.org/obo/GAZ_00002711"/>
        <obo:IAO_0000115>A populated place. A city in the Haifa District of Israel.</obo:IAO_0000115>
        <oboInOwl:hasOBONamespace>GAZ</oboInOwl:hasOBONamespace>
        <oboInOwl:id>GAZ:00078342</oboInOwl:id>
        <rdfs:label>City of Kiryat Atta</rdfs:label>
    </owl:NamedIndividual>
    


    <!-- http://purl.obolibrary.org/obo/GAZ_00078343 -->

    <owl:NamedIndividual rdf:about="http://purl.obolibrary.org/obo/GAZ_00078343">
        <obo:RO_0001025 rdf:resource="http://purl.obolibrary.org/obo/GAZ_00002711"/>
        <obo:IAO_0000115>A populated place. A city in the Haifa District in Israel.</obo:IAO_0000115>
        <oboInOwl:hasOBONamespace>GAZ</oboInOwl:hasOBONamespace>
        <oboInOwl:id>GAZ:00078343</oboInOwl:id>
        <rdfs:label>City of Nesher</rdfs:label>
    </owl:NamedIndividual>
    


    <!-- http://purl.obolibrary.org/obo/GAZ_00078344 -->

    <owl:NamedIndividual rdf:about="http://purl.obolibrary.org/obo/GAZ_00078344">
        <obo:RO_0001025 rdf:resource="http://purl.obolibrary.org/obo/GAZ_00002711"/>
        <obo:IAO_0000115>A city located in the Haifa District of Israel, on the country&apos;s Coastal Plain. It is located just inland from the ancient port city of Caesarea and the Mediterranean, and to the north of the city of Hadera. It is 30 miles south of Haifa and 24 miles north of Tel Aviv.</obo:IAO_0000115>
        <oboInOwl:hasOBONamespace>GAZ</oboInOwl:hasOBONamespace>
        <oboInOwl:id>GAZ:00078344</oboInOwl:id>
        <rdfs:label>City of Or Akiva</rdfs:label>
    </owl:NamedIndividual>
    


    <!-- http://purl.obolibrary.org/obo/GAZ_00078345 -->

    <owl:NamedIndividual rdf:about="http://purl.obolibrary.org/obo/GAZ_00078345">
        <obo:RO_0001025 rdf:resource="http://purl.obolibrary.org/obo/GAZ_00002711"/>
        <obo:IAO_0000115>An Israeli Arab city in the Haifa District of Israel.</obo:IAO_0000115>
        <oboInOwl:hasOBONamespace>GAZ</oboInOwl:hasOBONamespace>
        <oboInOwl:id>GAZ:00078345</oboInOwl:id>
        <rdfs:label>City of Umm al-Fahm</rdfs:label>
    </owl:NamedIndividual>
    


    <!-- http://purl.obolibrary.org/obo/GAZ_00078346 -->

    <owl:NamedIndividual rdf:about="http://purl.obolibrary.org/obo/GAZ_00078346">
        <obo:RO_0001025 rdf:resource="http://purl.obolibrary.org/obo/GAZ_00078176"/>
        <obo:IAO_0000115>A Local Council that is a suburb of Jerusalem, Israel. Today, Mevaseret Zion is composed of two distinct settlements - Maoz Zion and Mevaseret Yerushalayim - under the jurisdiction of one local council.</obo:IAO_0000115>
        <oboInOwl:hasOBONamespace>GAZ</oboInOwl:hasOBONamespace>
        <oboInOwl:id>GAZ:00078346</oboInOwl:id>
        <rdfs:label>Mevaseret Zion Local Council</rdfs:label>
    </owl:NamedIndividual>
    


    <!-- http://purl.obolibrary.org/obo/GAZ_00078347 -->

    <owl:NamedIndividual rdf:about="http://purl.obolibrary.org/obo/GAZ_00078347">
        <obo:RO_0001025 rdf:resource="http://purl.obolibrary.org/obo/GAZ_00078176"/>
        <obo:IAO_0000115>A Local Council in the Jerusalem District of Israel.</obo:IAO_0000115>
        <oboInOwl:hasOBONamespace>GAZ</oboInOwl:hasOBONamespace>
        <oboInOwl:id>GAZ:00078347</oboInOwl:id>
        <rdfs:label>Kiryat Ye&apos;arim Local Council</rdfs:label>
    </owl:NamedIndividual>
    


    <!-- http://purl.obolibrary.org/obo/GAZ_00078348 -->

    <owl:NamedIndividual rdf:about="http://purl.obolibrary.org/obo/GAZ_00078348">
        <obo:RO_0001025 rdf:resource="http://purl.obolibrary.org/obo/GAZ_00078176"/>
        <obo:IAO_0000115>A populated place. A city in Israel&apos;s Jerusalem District.</obo:IAO_0000115>
        <oboInOwl:hasOBONamespace>GAZ</oboInOwl:hasOBONamespace>
        <oboInOwl:id>GAZ:00078348</oboInOwl:id>
        <rdfs:label>City of Beit Shemesh</rdfs:label>
    </owl:NamedIndividual>
    


    <!-- http://purl.obolibrary.org/obo/GAZ_00078349 -->

    <owl:NamedIndividual rdf:about="http://purl.obolibrary.org/obo/GAZ_00078349">
        <obo:RO_0001025 rdf:resource="http://purl.obolibrary.org/obo/GAZ_00078176"/>
        <obo:IAO_0000115>An Israeli Arab Local Council west of Jerusalem on the road to Tel Aviv.</obo:IAO_0000115>
        <oboInOwl:hasOBONamespace>GAZ</oboInOwl:hasOBONamespace>
        <oboInOwl:id>GAZ:00078349</oboInOwl:id>
        <rdfs:label>Abu Ghosh Local Council</rdfs:label>
    </owl:NamedIndividual>
    


    <!-- http://purl.obolibrary.org/obo/GAZ_00078350 -->

    <owl:NamedIndividual rdf:about="http://purl.obolibrary.org/obo/GAZ_00078350">
        <obo:RO_0001025 rdf:resource="http://purl.obolibrary.org/obo/GAZ_00078176"/>
        <obo:IAO_0000115>A city located in the Judean Mountains, between the Mediterranean Sea and the northern tip of the Dead Sea.</obo:IAO_0000115>
        <oboInOwl:hasOBONamespace>GAZ</oboInOwl:hasOBONamespace>
        <oboInOwl:id>GAZ:00078350</oboInOwl:id>
        <rdfs:label>City of Jerusalem</rdfs:label>
    </owl:NamedIndividual>
    


    <!-- http://purl.obolibrary.org/obo/GAZ_00078351 -->

    <owl:NamedIndividual rdf:about="http://purl.obolibrary.org/obo/GAZ_00078351">
        <obo:RO_0001025 rdf:resource="http://purl.obolibrary.org/obo/GAZ_00002713"/>
        <obo:IAO_0000115>A regional council in the western Galilee of northern Israel.</obo:IAO_0000115>
        <oboInOwl:hasOBONamespace>GAZ</oboInOwl:hasOBONamespace>
        <oboInOwl:id>GAZ:00078351</oboInOwl:id>
        <rdfs:label>Matte Asher Regional Council</rdfs:label>
    </owl:NamedIndividual>
    


    <!-- http://purl.obolibrary.org/obo/GAZ_00078352 -->

    <owl:NamedIndividual rdf:about="http://purl.obolibrary.org/obo/GAZ_00078352">
        <obo:RO_0001025 rdf:resource="http://purl.obolibrary.org/obo/GAZ_00002713"/>
        <obo:IAO_0000115>A populated place. A city in the North District in Israel.</obo:IAO_0000115>
        <oboInOwl:hasOBONamespace>GAZ</oboInOwl:hasOBONamespace>
        <oboInOwl:id>GAZ:00078352</oboInOwl:id>
        <rdfs:label>City of Shefa-&apos;Amr</rdfs:label>
    </owl:NamedIndividual>
    


    <!-- http://purl.obolibrary.org/obo/GAZ_00078353 -->

    <owl:NamedIndividual rdf:about="http://purl.obolibrary.org/obo/GAZ_00078353">
        <obo:RO_0001025 rdf:resource="http://purl.obolibrary.org/obo/GAZ_00002713"/>
        <obo:IAO_0000115>A regional council in the Galilee region in the north of Israel.</obo:IAO_0000115>
        <oboInOwl:hasOBONamespace>GAZ</oboInOwl:hasOBONamespace>
        <oboInOwl:id>GAZ:00078353</oboInOwl:id>
        <rdfs:label>Misgav Regional Council</rdfs:label>
    </owl:NamedIndividual>
    


    <!-- http://purl.obolibrary.org/obo/GAZ_00078354 -->

    <owl:NamedIndividual rdf:about="http://purl.obolibrary.org/obo/GAZ_00078354">
        <obo:RO_0001025 rdf:resource="http://purl.obolibrary.org/obo/GAZ_00002713"/>
        <obo:IAO_0000115>An Israeli-Arab city in the North District of Israel located east of the coastal city of Acre (Akka). It was formed in 2003 with the merger of three Arab local councils - Majd al-Krum, Deir al-Asad and Bi&apos;ina.</obo:IAO_0000115>
        <oboInOwl:hasOBONamespace>GAZ</oboInOwl:hasOBONamespace>
        <oboInOwl:id>GAZ:00078354</oboInOwl:id>
        <rdfs:label>City of Shaghur</rdfs:label>
    </owl:NamedIndividual>
    


    <!-- http://purl.obolibrary.org/obo/GAZ_00078355 -->

    <owl:NamedIndividual rdf:about="http://purl.obolibrary.org/obo/GAZ_00078355">
        <obo:RO_0001025 rdf:resource="http://purl.obolibrary.org/obo/GAZ_00002713"/>
        <obo:IAO_0000115>A ridge above the Jezreel Valley in northern Israel. The ridge extends southeast-northwest from the Samarian highlands, and separates between Jenin and the Beit She&apos;an valley.</obo:IAO_0000115>
        <oboInOwl:hasOBONamespace>GAZ</oboInOwl:hasOBONamespace>
        <oboInOwl:id>GAZ:00078355</oboInOwl:id>
        <rdfs:label>Gilboa Ridge</rdfs:label>
    </owl:NamedIndividual>
    


    <!-- http://purl.obolibrary.org/obo/GAZ_00078356 -->

    <owl:NamedIndividual rdf:about="http://purl.obolibrary.org/obo/GAZ_00078356">
        <obo:RO_0001025 rdf:resource="http://purl.obolibrary.org/obo/GAZ_00002713"/>
        <obo:IAO_0000115>A regional council in the Jordan River Valley between the Sea of Galilee in the north and Bet Shean in the south.</obo:IAO_0000115>
        <oboInOwl:hasOBONamespace>GAZ</oboInOwl:hasOBONamespace>
        <oboInOwl:id>GAZ:00078356</oboInOwl:id>
        <rdfs:label>Emek HaYarden Regional Council</rdfs:label>
    </owl:NamedIndividual>
    


    <!-- http://purl.obolibrary.org/obo/GAZ_00078357 -->

    <owl:NamedIndividual rdf:about="http://purl.obolibrary.org/obo/GAZ_00078357">
        <obo:RO_0001025 rdf:resource="http://purl.obolibrary.org/obo/GAZ_00002713"/>
        <obo:IAO_0000115>A regional council in northern Israel that encompasses most of the settlements in the Beit She&apos;an Valley. The territory of the regional council is bounded by the Jezreel Valley in the west, in the north by the Lower Galilee, to the east by the Jordan River, and the south by the Jordan Valley and Samarian hills.</obo:IAO_0000115>
        <oboInOwl:hasOBONamespace>GAZ</oboInOwl:hasOBONamespace>
        <oboInOwl:id>GAZ:00078357</oboInOwl:id>
        <rdfs:label>Beit She&apos;an Valley Regional Council</rdfs:label>
    </owl:NamedIndividual>
    


    <!-- http://purl.obolibrary.org/obo/GAZ_00078358 -->

    <owl:NamedIndividual rdf:about="http://purl.obolibrary.org/obo/GAZ_00078358">
        <obo:RO_0001025 rdf:resource="http://purl.obolibrary.org/obo/GAZ_00002713"/>
        <obo:IAO_0000115>A regional council in northern Israel encompassing land on the Menashe Plateau, and partly in the Jezreel Valley. The council is bounded by the city of Yokneam Illit to the north, and the Carmel mountain range to the east.</obo:IAO_0000115>
        <oboInOwl:hasOBONamespace>GAZ</oboInOwl:hasOBONamespace>
        <oboInOwl:id>GAZ:00078358</oboInOwl:id>
        <rdfs:label>Megiddo Regional Council</rdfs:label>
    </owl:NamedIndividual>
    


    <!-- http://purl.obolibrary.org/obo/GAZ_00078359 -->

    <owl:NamedIndividual rdf:about="http://purl.obolibrary.org/obo/GAZ_00078359">
        <obo:RO_0001025 rdf:resource="http://purl.obolibrary.org/obo/GAZ_00002713"/>
        <obo:IAO_0000115>A populated place. A city in the North District of Israel.</obo:IAO_0000115>
        <oboInOwl:hasOBONamespace>GAZ</oboInOwl:hasOBONamespace>
        <oboInOwl:id>GAZ:00078359</oboInOwl:id>
        <rdfs:label>City of Nazareth Illit</rdfs:label>
    </owl:NamedIndividual>
    


    <!-- http://purl.obolibrary.org/obo/GAZ_00078360 -->

    <owl:NamedIndividual rdf:about="http://purl.obolibrary.org/obo/GAZ_00078360">
        <obo:RO_0001025 rdf:resource="http://purl.obolibrary.org/obo/GAZ_00002713"/>
        <obo:IAO_0000115>A regional council in the northern Galilee of northern Israel. The regional council was established in 1950.</obo:IAO_0000115>
        <oboInOwl:hasOBONamespace>GAZ</oboInOwl:hasOBONamespace>
        <oboInOwl:id>GAZ:00078360</oboInOwl:id>
        <rdfs:label>Merom HaGalil Regional Council</rdfs:label>
    </owl:NamedIndividual>
    


    <!-- http://purl.obolibrary.org/obo/GAZ_00078361 -->

    <owl:NamedIndividual rdf:about="http://purl.obolibrary.org/obo/GAZ_00078361">
        <obo:RO_0001025 rdf:resource="http://purl.obolibrary.org/obo/GAZ_00002713"/>
        <obo:IAO_0000115>A regional council in northern Israel, located on the slopes of the Gilboa mountain range.</obo:IAO_0000115>
        <oboInOwl:hasOBONamespace>GAZ</oboInOwl:hasOBONamespace>
        <oboInOwl:id>GAZ:00078361</oboInOwl:id>
        <rdfs:label>Gilboa Regional Council</rdfs:label>
    </owl:NamedIndividual>
    


    <!-- http://purl.obolibrary.org/obo/GAZ_00078362 -->

    <owl:NamedIndividual rdf:about="http://purl.obolibrary.org/obo/GAZ_00078362">
        <obo:RO_0001025 rdf:resource="http://purl.obolibrary.org/obo/GAZ_00002713"/>
        <oboInOwl:hasOBONamespace>GAZ</oboInOwl:hasOBONamespace>
        <oboInOwl:id>GAZ:00078362</oboInOwl:id>
        <rdfs:label>City of Ma&apos;alot-Tarshiha</rdfs:label>
    </owl:NamedIndividual>
    


    <!-- http://purl.obolibrary.org/obo/GAZ_00078363 -->

    <owl:NamedIndividual rdf:about="http://purl.obolibrary.org/obo/GAZ_00078363">
        <obo:RO_0001025 rdf:resource="http://purl.obolibrary.org/obo/GAZ_00002713"/>
        <obo:IAO_0000115>The regional council consolidating virtually all the Jewish Israeli settlements located on the Golan Heights. It is made up of 19 moshavim and 10 kibbutzim, and other villages. While the headquarters are located in the town of Katzrin, that town is itself an independent local council.</obo:IAO_0000115>
        <oboInOwl:hasOBONamespace>GAZ</oboInOwl:hasOBONamespace>
        <oboInOwl:id>GAZ:00078363</oboInOwl:id>
        <rdfs:label>Golan Regional Council</rdfs:label>
    </owl:NamedIndividual>
    


    <!-- http://purl.obolibrary.org/obo/GAZ_00078364 -->

    <owl:NamedIndividual rdf:about="http://purl.obolibrary.org/obo/GAZ_00078364">
        <obo:RO_0001025 rdf:resource="http://purl.obolibrary.org/obo/GAZ_00002713"/>
        <obo:IAO_0000115>A Regional Council located on the southern fringe of the Bet Netofa Valley in the North District of Israel.</obo:IAO_0000115>
        <oboInOwl:hasOBONamespace>GAZ</oboInOwl:hasOBONamespace>
        <oboInOwl:id>GAZ:00078364</oboInOwl:id>
        <rdfs:label>al-Batuf Regional Council</rdfs:label>
    </owl:NamedIndividual>
    


    <!-- http://purl.obolibrary.org/obo/GAZ_00078365 -->

    <owl:NamedIndividual rdf:about="http://purl.obolibrary.org/obo/GAZ_00078365">
        <obo:RO_0001025 rdf:resource="http://purl.obolibrary.org/obo/GAZ_00002713"/>
        <obo:IAO_0000115>A Regional Council in the North District of Israel. It encompasses 13 Moshavim and Communal settlements, from the northern shore of the Kinneret, to the Lebanese border and Mount Hermon.</obo:IAO_0000115>
        <oboInOwl:hasOBONamespace>GAZ</oboInOwl:hasOBONamespace>
        <oboInOwl:id>GAZ:00078365</oboInOwl:id>
        <rdfs:label>Mevo&apos;ot HaHermon Regional Council</rdfs:label>
    </owl:NamedIndividual>
    


    <!-- http://purl.obolibrary.org/obo/GAZ_00078366 -->

    <owl:NamedIndividual rdf:about="http://purl.obolibrary.org/obo/GAZ_00078366">
        <obo:RO_0001025 rdf:resource="http://purl.obolibrary.org/obo/GAZ_00002713"/>
        <obo:IAO_0000115>A regional council in northern Israel. Its territory lies adjacent to the Jezreel Valley and north of Afula.</obo:IAO_0000115>
        <oboInOwl:hasOBONamespace>GAZ</oboInOwl:hasOBONamespace>
        <oboInOwl:id>GAZ:00078366</oboInOwl:id>
        <rdfs:label>Bustan al-Marj Regional Council</rdfs:label>
    </owl:NamedIndividual>
    


    <!-- http://purl.obolibrary.org/obo/GAZ_00078367 -->

    <owl:NamedIndividual rdf:about="http://purl.obolibrary.org/obo/GAZ_00078367">
        <obo:RO_0001025 rdf:resource="http://purl.obolibrary.org/obo/GAZ_00002713"/>
        <obo:IAO_0000115>A regional council in the Upper Galilee, part of the North District of Israel, situated between the towns of Ma&apos;alot-Tarshiha and Shlomi.</obo:IAO_0000115>
        <oboInOwl:hasOBONamespace>GAZ</oboInOwl:hasOBONamespace>
        <oboInOwl:id>GAZ:00078367</oboInOwl:id>
        <rdfs:label>Ma&apos;ale Yosef Regional Council</rdfs:label>
    </owl:NamedIndividual>
    


    <!-- http://purl.obolibrary.org/obo/GAZ_00078368 -->

    <owl:NamedIndividual rdf:about="http://purl.obolibrary.org/obo/GAZ_00078368">
        <obo:RO_0001025 rdf:resource="http://purl.obolibrary.org/obo/GAZ_00002713"/>
        <oboInOwl:hasOBONamespace>GAZ</oboInOwl:hasOBONamespace>
        <oboInOwl:id>GAZ:00078368</oboInOwl:id>
        <rdfs:label>City of Kiryat Shmona</rdfs:label>
    </owl:NamedIndividual>
    


    <!-- http://purl.obolibrary.org/obo/GAZ_00078369 -->

    <owl:NamedIndividual rdf:about="http://purl.obolibrary.org/obo/GAZ_00078369">
        <obo:RO_0001025 rdf:resource="http://purl.obolibrary.org/obo/GAZ_00002713"/>
        <obo:IAO_0000115>A populated place. A city in the Northern District of Israel.</obo:IAO_0000115>
        <oboInOwl:hasOBONamespace>GAZ</oboInOwl:hasOBONamespace>
        <oboInOwl:id>GAZ:00078369</oboInOwl:id>
        <rdfs:label>City of Safed</rdfs:label>
    </owl:NamedIndividual>
    


    <!-- http://purl.obolibrary.org/obo/GAZ_00078370 -->

    <owl:NamedIndividual rdf:about="http://purl.obolibrary.org/obo/GAZ_00078370">
        <obo:RO_0001025 rdf:resource="http://purl.obolibrary.org/obo/GAZ_00002713"/>
        <obo:IAO_0000115>The capital and largest city in the North District of Israel.</obo:IAO_0000115>
        <oboInOwl:hasOBONamespace>GAZ</oboInOwl:hasOBONamespace>
        <oboInOwl:id>GAZ:00078370</oboInOwl:id>
        <rdfs:label>City of Nazareth</rdfs:label>
    </owl:NamedIndividual>
    


    <!-- http://purl.obolibrary.org/obo/GAZ_00078371 -->

    <owl:NamedIndividual rdf:about="http://purl.obolibrary.org/obo/GAZ_00078371">
        <obo:RO_0001025 rdf:resource="http://purl.obolibrary.org/obo/GAZ_00002713"/>
        <obo:IAO_0000115>A populated place. A city in the North District of Israel at the junction of the Jordan River Valley and Jezreel Valley.</obo:IAO_0000115>
        <oboInOwl:hasOBONamespace>GAZ</oboInOwl:hasOBONamespace>
        <oboInOwl:id>GAZ:00078371</oboInOwl:id>
        <rdfs:label>City of Bet She&apos;an</rdfs:label>
    </owl:NamedIndividual>
    


    <!-- http://purl.obolibrary.org/obo/GAZ_00078372 -->

    <owl:NamedIndividual rdf:about="http://purl.obolibrary.org/obo/GAZ_00078372">
        <obo:RO_0001025 rdf:resource="http://purl.obolibrary.org/obo/GAZ_00002713"/>
        <oboInOwl:hasOBONamespace>GAZ</oboInOwl:hasOBONamespace>
        <oboInOwl:id>GAZ:00078372</oboInOwl:id>
        <rdfs:label>City of Migdal HaEmek</rdfs:label>
    </owl:NamedIndividual>
    


    <!-- http://purl.obolibrary.org/obo/GAZ_00078373 -->

    <owl:NamedIndividual rdf:about="http://purl.obolibrary.org/obo/GAZ_00078373">
        <obo:RO_0001025 rdf:resource="http://purl.obolibrary.org/obo/GAZ_00002713"/>
        <obo:IAO_0000115>An Israeli Arab city in the North District of Israel located in the Lower Galilee 5 km north of the city of Shefa-&apos;Amr and approximately 20 km east of Akko (Acre).</obo:IAO_0000115>
        <oboInOwl:hasOBONamespace>GAZ</oboInOwl:hasOBONamespace>
        <oboInOwl:id>GAZ:00078373</oboInOwl:id>
        <rdfs:label>City of Tamra</rdfs:label>
    </owl:NamedIndividual>
    


    <!-- http://purl.obolibrary.org/obo/GAZ_00078374 -->

    <owl:NamedIndividual rdf:about="http://purl.obolibrary.org/obo/GAZ_00078374">
        <obo:RO_0001025 rdf:resource="http://purl.obolibrary.org/obo/GAZ_00002713"/>
        <obo:IAO_0000115>An Arab Israeli city in Israel&apos;s North District. It is located in the Lower Galilee, about 23 km east of Acre.</obo:IAO_0000115>
        <oboInOwl:hasOBONamespace>GAZ</oboInOwl:hasOBONamespace>
        <oboInOwl:id>GAZ:00078374</oboInOwl:id>
        <rdfs:label>City of Sakhnin</rdfs:label>
    </owl:NamedIndividual>
    


    <!-- http://purl.obolibrary.org/obo/GAZ_00078375 -->

    <owl:NamedIndividual rdf:about="http://purl.obolibrary.org/obo/GAZ_00078375">
        <obo:RO_0001025 rdf:resource="http://purl.obolibrary.org/obo/GAZ_00002713"/>
        <obo:IAO_0000115>A city on the western shore of the Sea of Galilee, Lower Galilee, Israel.</obo:IAO_0000115>
        <oboInOwl:hasOBONamespace>GAZ</oboInOwl:hasOBONamespace>
        <oboInOwl:id>GAZ:00078375</oboInOwl:id>
        <rdfs:label>City of Tiberias</rdfs:label>
    </owl:NamedIndividual>
    


    <!-- http://purl.obolibrary.org/obo/GAZ_00078376 -->

    <owl:NamedIndividual rdf:about="http://purl.obolibrary.org/obo/GAZ_00078376">
        <obo:RO_0001025 rdf:resource="http://purl.obolibrary.org/obo/GAZ_00002713"/>
        <oboInOwl:hasOBONamespace>GAZ</oboInOwl:hasOBONamespace>
        <oboInOwl:id>GAZ:00078376</oboInOwl:id>
        <rdfs:label>City of Karmiel</rdfs:label>
    </owl:NamedIndividual>
    


    <!-- http://purl.obolibrary.org/obo/GAZ_00078377 -->

    <owl:NamedIndividual rdf:about="http://purl.obolibrary.org/obo/GAZ_00078377">
        <obo:RO_0001025 rdf:resource="http://purl.obolibrary.org/obo/GAZ_00002713"/>
        <obo:IAO_0000115>A small city council southeast of Haifa in northern Israel. It is located in a hilly region of northern Israel&apos;s lower Galilee, bordered by Highway 70 and Mount Carmel.</obo:IAO_0000115>
        <oboInOwl:hasOBONamespace>GAZ</oboInOwl:hasOBONamespace>
        <oboInOwl:id>GAZ:00078377</oboInOwl:id>
        <rdfs:label>City of Yokneam</rdfs:label>
    </owl:NamedIndividual>
    


    <!-- http://purl.obolibrary.org/obo/GAZ_00078378 -->

    <owl:NamedIndividual rdf:about="http://purl.obolibrary.org/obo/GAZ_00078378">
        <obo:RO_0001025 rdf:resource="http://purl.obolibrary.org/obo/GAZ_00002713"/>
        <obo:IAO_0000115>A populated place. A city in the North District of Israel.</obo:IAO_0000115>
        <oboInOwl:hasOBONamespace>GAZ</oboInOwl:hasOBONamespace>
        <oboInOwl:id>GAZ:00078378</oboInOwl:id>
        <rdfs:label>City of Afula</rdfs:label>
    </owl:NamedIndividual>
    


    <!-- http://purl.obolibrary.org/obo/GAZ_00078379 -->

    <owl:NamedIndividual rdf:about="http://purl.obolibrary.org/obo/GAZ_00078379">
        <obo:RO_0001025 rdf:resource="http://purl.obolibrary.org/obo/GAZ_00002713"/>
        <obo:IAO_0000115>A populated place. A city in the Western Galilee district of northern Israel. It is situated on a low promontory at the northern extremity of Haifa Bay.</obo:IAO_0000115>
        <oboInOwl:hasOBONamespace>GAZ</oboInOwl:hasOBONamespace>
        <oboInOwl:id>GAZ:00078379</oboInOwl:id>
        <rdfs:label>City of Acre</rdfs:label>
    </owl:NamedIndividual>
    


    <!-- http://purl.obolibrary.org/obo/GAZ_00078380 -->

    <owl:NamedIndividual rdf:about="http://purl.obolibrary.org/obo/GAZ_00078380">
        <obo:RO_0001025 rdf:resource="http://purl.obolibrary.org/obo/GAZ_00002713"/>
        <obo:IAO_0000115>A Druze local council in the Northern District of Israel. It was declared a local council in 1967.</obo:IAO_0000115>
        <oboInOwl:hasOBONamespace>GAZ</oboInOwl:hasOBONamespace>
        <oboInOwl:id>GAZ:00078380</oboInOwl:id>
        <rdfs:label>Hurfeish Local Council</rdfs:label>
    </owl:NamedIndividual>
    


    <!-- http://purl.obolibrary.org/obo/GAZ_00078381 -->

    <owl:NamedIndividual rdf:about="http://purl.obolibrary.org/obo/GAZ_00078381">
        <obo:RO_0001025 rdf:resource="http://purl.obolibrary.org/obo/GAZ_00002713"/>
        <obo:IAO_0000115>An Arab Local Council in the Galilee region of Israel.</obo:IAO_0000115>
        <oboInOwl:hasOBONamespace>GAZ</oboInOwl:hasOBONamespace>
        <oboInOwl:id>GAZ:00078381</oboInOwl:id>
        <rdfs:label>Kafr Kanna Local Council</rdfs:label>
    </owl:NamedIndividual>
    


    <!-- http://purl.obolibrary.org/obo/GAZ_00078382 -->

    <owl:NamedIndividual rdf:about="http://purl.obolibrary.org/obo/GAZ_00078382">
        <obo:RO_0001025 rdf:resource="http://purl.obolibrary.org/obo/GAZ_00078363"/>
        <obo:IAO_0000115>A kibbutz in the southern Golan Heights. The southernmost village in the Golan, it is located 2 km from the Sea of Galilee at a height of 350 meters above sea level, it falls under the jurisdiction of Golan Regional Council.</obo:IAO_0000115>
        <oboInOwl:hasOBONamespace>GAZ</oboInOwl:hasOBONamespace>
        <oboInOwl:id>GAZ:00078382</oboInOwl:id>
        <rdfs:label>Mevo Hama</rdfs:label>
    </owl:NamedIndividual>
    


    <!-- http://purl.obolibrary.org/obo/GAZ_00078383 -->

    <owl:NamedIndividual rdf:about="http://purl.obolibrary.org/obo/GAZ_00078383">
        <obo:RO_0001025 rdf:resource="http://purl.obolibrary.org/obo/GAZ_00002713"/>
        <obo:IAO_0000115>An Arab local council in the North District of Israel. It was declared a local council in 1991.</obo:IAO_0000115>
        <oboInOwl:hasOBONamespace>GAZ</oboInOwl:hasOBONamespace>
        <oboInOwl:id>GAZ:00078383</oboInOwl:id>
        <rdfs:label>Ilut Local Council</rdfs:label>
    </owl:NamedIndividual>
    


    <!-- http://purl.obolibrary.org/obo/GAZ_00078384 -->

    <owl:NamedIndividual rdf:about="http://purl.obolibrary.org/obo/GAZ_00078384">
        <obo:RO_0001025 rdf:resource="http://purl.obolibrary.org/obo/GAZ_00002713"/>
        <obo:IAO_0000115>A Local Council in the Lower Galilee region of northern Israel, at the foot of Mount Tabor.</obo:IAO_0000115>
        <oboInOwl:hasOBONamespace>GAZ</oboInOwl:hasOBONamespace>
        <oboInOwl:id>GAZ:00078384</oboInOwl:id>
        <rdfs:label>Kfar Tavor Local Council</rdfs:label>
    </owl:NamedIndividual>
    


    <!-- http://purl.obolibrary.org/obo/GAZ_00078385 -->

    <owl:NamedIndividual rdf:about="http://purl.obolibrary.org/obo/GAZ_00078385">
        <obo:RO_0001025 rdf:resource="http://purl.obolibrary.org/obo/GAZ_00002713"/>
        <obo:IAO_0000115>An Israeli Arab local council formed by the merger of the two Arab towns of Makr and Jadeidi in 1990. It is located a few km east of the city of Acre in the North District.</obo:IAO_0000115>
        <oboInOwl:hasOBONamespace>GAZ</oboInOwl:hasOBONamespace>
        <oboInOwl:id>GAZ:00078385</oboInOwl:id>
        <rdfs:label>Jadeidi-Makr Local Council</rdfs:label>
    </owl:NamedIndividual>
    


    <!-- http://purl.obolibrary.org/obo/GAZ_00078386 -->

    <owl:NamedIndividual rdf:about="http://purl.obolibrary.org/obo/GAZ_00078386">
        <obo:RO_0001025 rdf:resource="http://purl.obolibrary.org/obo/GAZ_00002713"/>
        <obo:IAO_0000115>A Local Council in the Northen District of Israel.</obo:IAO_0000115>
        <oboInOwl:hasOBONamespace>GAZ</oboInOwl:hasOBONamespace>
        <oboInOwl:id>GAZ:00078386</oboInOwl:id>
        <rdfs:label>Ma&apos;ar Local Council</rdfs:label>
    </owl:NamedIndividual>
    


    <!-- http://purl.obolibrary.org/obo/GAZ_00078387 -->

    <owl:NamedIndividual rdf:about="http://purl.obolibrary.org/obo/GAZ_00078387">
        <obo:RO_0001025 rdf:resource="http://purl.obolibrary.org/obo/GAZ_00002713"/>
        <obo:IAO_0000115>A Local Council in the Northern District of Israel.</obo:IAO_0000115>
        <oboInOwl:hasOBONamespace>GAZ</oboInOwl:hasOBONamespace>
        <oboInOwl:id>GAZ:00078387</oboInOwl:id>
        <rdfs:label>Mi&apos;elya Local Council</rdfs:label>
    </owl:NamedIndividual>
    


    <!-- http://purl.obolibrary.org/obo/GAZ_00078388 -->

    <owl:NamedIndividual rdf:about="http://purl.obolibrary.org/obo/GAZ_00078388">
        <obo:RO_0001025 rdf:resource="http://purl.obolibrary.org/obo/GAZ_00002713"/>
        <obo:IAO_0000115>An Arab Local Council located on the northeastern slopes of Mt. Meron, 13 km north of Safed in Israel&apos;s North District.</obo:IAO_0000115>
        <oboInOwl:hasOBONamespace>GAZ</oboInOwl:hasOBONamespace>
        <oboInOwl:id>GAZ:00078388</oboInOwl:id>
        <rdfs:label>Jish Local Council</rdfs:label>
    </owl:NamedIndividual>
    


    <!-- http://purl.obolibrary.org/obo/GAZ_00078389 -->

    <owl:NamedIndividual rdf:about="http://purl.obolibrary.org/obo/GAZ_00078389">
        <obo:RO_0001025 rdf:resource="http://purl.obolibrary.org/obo/GAZ_00002713"/>
        <obo:IAO_0000115>A Local Council in the Northern District of Israel.</obo:IAO_0000115>
        <oboInOwl:hasOBONamespace>GAZ</oboInOwl:hasOBONamespace>
        <oboInOwl:id>GAZ:00078389</oboInOwl:id>
        <rdfs:label>Kinneret Local Council</rdfs:label>
    </owl:NamedIndividual>
    


    <!-- http://purl.obolibrary.org/obo/GAZ_00078390 -->

    <owl:NamedIndividual rdf:about="http://purl.obolibrary.org/obo/GAZ_00078390">
        <obo:RO_0001025 rdf:resource="http://purl.obolibrary.org/obo/GAZ_00002713"/>
        <obo:IAO_0000115>An Israeli-Arab local council located 10 km west of the city of Nazareth in Israel&apos;s North District. It became a local council in 1997.</obo:IAO_0000115>
        <oboInOwl:hasOBONamespace>GAZ</oboInOwl:hasOBONamespace>
        <oboInOwl:id>GAZ:00078390</oboInOwl:id>
        <rdfs:label>Zarzir Local Council</rdfs:label>
    </owl:NamedIndividual>
    


    <!-- http://purl.obolibrary.org/obo/GAZ_00078391 -->

    <owl:NamedIndividual rdf:about="http://purl.obolibrary.org/obo/GAZ_00078391">
        <obo:RO_0001025 rdf:resource="http://purl.obolibrary.org/obo/GAZ_00002713"/>
        <obo:IAO_0000115>A Local Council in the Northern District of Israel.</obo:IAO_0000115>
        <oboInOwl:hasOBONamespace>GAZ</oboInOwl:hasOBONamespace>
        <oboInOwl:id>GAZ:00078391</oboInOwl:id>
        <rdfs:label>Kaokab Abu al-Hija Local Council</rdfs:label>
    </owl:NamedIndividual>
    


    <!-- http://purl.obolibrary.org/obo/GAZ_00078392 -->

    <owl:NamedIndividual rdf:about="http://purl.obolibrary.org/obo/GAZ_00078392">
        <obo:RO_0001025 rdf:resource="http://purl.obolibrary.org/obo/GAZ_00002713"/>
        <obo:IAO_0000115>A Local Council in the Northern District of Israel.</obo:IAO_0000115>
        <oboInOwl:hasOBONamespace>GAZ</oboInOwl:hasOBONamespace>
        <oboInOwl:id>GAZ:00078392</oboInOwl:id>
        <rdfs:label>Shlomi Local Council</rdfs:label>
    </owl:NamedIndividual>
    


    <!-- http://purl.obolibrary.org/obo/GAZ_00078393 -->

    <owl:NamedIndividual rdf:about="http://purl.obolibrary.org/obo/GAZ_00078393">
        <obo:RO_0001025 rdf:resource="http://purl.obolibrary.org/obo/GAZ_00002713"/>
        <obo:IAO_0000115>A local council in the Northern District of Israel. The municipality was established it 1960.</obo:IAO_0000115>
        <oboInOwl:hasOBONamespace>GAZ</oboInOwl:hasOBONamespace>
        <oboInOwl:id>GAZ:00078393</oboInOwl:id>
        <rdfs:label>I&apos;billin Local Council</rdfs:label>
    </owl:NamedIndividual>
    


    <!-- http://purl.obolibrary.org/obo/GAZ_00078394 -->

    <owl:NamedIndividual rdf:about="http://purl.obolibrary.org/obo/GAZ_00078394">
        <obo:RO_0001025 rdf:resource="http://purl.obolibrary.org/obo/GAZ_00002713"/>
        <obo:IAO_0000115>An Israeli-Arab local council in the North District of Israel. It is located a few km northeast of the city of Acre.</obo:IAO_0000115>
        <oboInOwl:hasOBONamespace>GAZ</oboInOwl:hasOBONamespace>
        <oboInOwl:id>GAZ:00078394</oboInOwl:id>
        <rdfs:label>Kafr Yasif Local Council</rdfs:label>
    </owl:NamedIndividual>
    


    <!-- http://purl.obolibrary.org/obo/GAZ_00078395 -->

    <owl:NamedIndividual rdf:about="http://purl.obolibrary.org/obo/GAZ_00078395">
        <obo:RO_0001025 rdf:resource="http://purl.obolibrary.org/obo/GAZ_00002713"/>
        <obo:IAO_0000115>An Israeli-Arab local council located in the Lower Galilee on the slopes of Mount Atzmon in the Israel&apos;s North District. It is 16 km northwest of the city of Nazareth.</obo:IAO_0000115>
        <oboInOwl:hasOBONamespace>GAZ</oboInOwl:hasOBONamespace>
        <oboInOwl:id>GAZ:00078395</oboInOwl:id>
        <rdfs:label>Kafr Manda Local Council</rdfs:label>
    </owl:NamedIndividual>
    


    <!-- http://purl.obolibrary.org/obo/GAZ_00078396 -->

    <owl:NamedIndividual rdf:about="http://purl.obolibrary.org/obo/GAZ_00078396">
        <obo:RO_0001025 rdf:resource="http://purl.obolibrary.org/obo/GAZ_00002713"/>
        <obo:IAO_0000115>A local council in the North District of Israel, located east of Acre and north of Shefa-&apos;Amr.</obo:IAO_0000115>
        <oboInOwl:hasOBONamespace>GAZ</oboInOwl:hasOBONamespace>
        <oboInOwl:id>GAZ:00078396</oboInOwl:id>
        <rdfs:label>Kabul Local Council</rdfs:label>
    </owl:NamedIndividual>
    


    <!-- http://purl.obolibrary.org/obo/GAZ_00078397 -->

    <owl:NamedIndividual rdf:about="http://purl.obolibrary.org/obo/GAZ_00078397">
        <obo:RO_0001025 rdf:resource="http://purl.obolibrary.org/obo/GAZ_00002713"/>
        <obo:IAO_0000115>An Israeli Arab local council) in northern Israel, about 1 km east of Nazareth Illit.</obo:IAO_0000115>
        <oboInOwl:hasOBONamespace>GAZ</oboInOwl:hasOBONamespace>
        <oboInOwl:id>GAZ:00078397</oboInOwl:id>
        <rdfs:label>Iksal Local Council</rdfs:label>
    </owl:NamedIndividual>
    


    <!-- http://purl.obolibrary.org/obo/GAZ_00078398 -->

    <owl:NamedIndividual rdf:about="http://purl.obolibrary.org/obo/GAZ_00078398">
        <obo:RO_0001025 rdf:resource="http://purl.obolibrary.org/obo/GAZ_00002713"/>
        <obo:IAO_0000115>A local council in northern Israel, next to Rosh Pina and near Safed.</obo:IAO_0000115>
        <oboInOwl:hasOBONamespace>GAZ</oboInOwl:hasOBONamespace>
        <oboInOwl:id>GAZ:00078398</oboInOwl:id>
        <rdfs:label>Hazor HaGelilit Local Council</rdfs:label>
    </owl:NamedIndividual>
    


    <!-- http://purl.obolibrary.org/obo/GAZ_00078399 -->

    <owl:NamedIndividual rdf:about="http://purl.obolibrary.org/obo/GAZ_00078399">
        <obo:RO_0001025 rdf:resource="http://purl.obolibrary.org/obo/GAZ_00002713"/>
        <obo:IAO_0000115>A Local Council in the Northern District of Israel.</obo:IAO_0000115>
        <oboInOwl:hasOBONamespace>GAZ</oboInOwl:hasOBONamespace>
        <oboInOwl:id>GAZ:00078399</oboInOwl:id>
        <rdfs:label>Kisra-Sume&apos;a Local Council</rdfs:label>
    </owl:NamedIndividual>
    


    <!-- http://purl.obolibrary.org/obo/GAZ_00078400 -->

    <owl:NamedIndividual rdf:about="http://purl.obolibrary.org/obo/GAZ_00078400">
        <obo:RO_0001025 rdf:resource="http://purl.obolibrary.org/obo/GAZ_00002713"/>
        <obo:IAO_0000115>A Bedouin local council in the North District of Israel. It was declared as a local council in 1965.</obo:IAO_0000115>
        <oboInOwl:hasOBONamespace>GAZ</oboInOwl:hasOBONamespace>
        <oboInOwl:id>GAZ:00078400</oboInOwl:id>
        <rdfs:label>Basmat Tab&apos;un Local Council</rdfs:label>
    </owl:NamedIndividual>
    


    <!-- http://purl.obolibrary.org/obo/GAZ_00078401 -->

    <owl:NamedIndividual rdf:about="http://purl.obolibrary.org/obo/GAZ_00078401">
        <obo:RO_0001025 rdf:resource="http://purl.obolibrary.org/obo/GAZ_00002713"/>
        <obo:IAO_0000115>A local council in the North District of Israel, located on the hills of the Lower Galilee, 23 km southeast of Acre.</obo:IAO_0000115>
        <oboInOwl:hasOBONamespace>GAZ</oboInOwl:hasOBONamespace>
        <oboInOwl:id>GAZ:00078401</oboInOwl:id>
        <rdfs:label>Deir Hanna Local Council</rdfs:label>
    </owl:NamedIndividual>
    


    <!-- http://purl.obolibrary.org/obo/GAZ_00078402 -->

    <owl:NamedIndividual rdf:about="http://purl.obolibrary.org/obo/GAZ_00078402">
        <obo:RO_0001025 rdf:resource="http://purl.obolibrary.org/obo/GAZ_00002713"/>
        <obo:IAO_0000115>An Arab local council in the North District of Israel. It was declared as a local council in 1996.</obo:IAO_0000115>
        <oboInOwl:hasOBONamespace>GAZ</oboInOwl:hasOBONamespace>
        <oboInOwl:id>GAZ:00078402</oboInOwl:id>
        <rdfs:label>Bu&apos;eine Nujeidat Local Council</rdfs:label>
    </owl:NamedIndividual>
    


    <!-- http://purl.obolibrary.org/obo/GAZ_00078403 -->

    <owl:NamedIndividual rdf:about="http://purl.obolibrary.org/obo/GAZ_00078403">
        <obo:RO_0001025 rdf:resource="http://purl.obolibrary.org/obo/GAZ_00002713"/>
        <obo:IAO_0000115>A Druze local council in the Golan Heights. It was declared a local council in 1982.</obo:IAO_0000115>
        <oboInOwl:hasOBONamespace>GAZ</oboInOwl:hasOBONamespace>
        <oboInOwl:id>GAZ:00078403</oboInOwl:id>
        <rdfs:label>Ein Qiniyye Local Council</rdfs:label>
    </owl:NamedIndividual>
    


    <!-- http://purl.obolibrary.org/obo/GAZ_00078404 -->

    <owl:NamedIndividual rdf:about="http://purl.obolibrary.org/obo/GAZ_00078404">
        <obo:RO_0001025 rdf:resource="http://purl.obolibrary.org/obo/GAZ_00002713"/>
        <obo:IAO_0000115>A Local Council in Israel&apos;s North District.</obo:IAO_0000115>
        <oboInOwl:hasOBONamespace>GAZ</oboInOwl:hasOBONamespace>
        <oboInOwl:id>GAZ:00078404</oboInOwl:id>
        <rdfs:label>Daburiyya Local Council</rdfs:label>
    </owl:NamedIndividual>
    


    <!-- http://purl.obolibrary.org/obo/GAZ_00078405 -->

    <owl:NamedIndividual rdf:about="http://purl.obolibrary.org/obo/GAZ_00078405">
        <obo:RO_0001025 rdf:resource="http://purl.obolibrary.org/obo/GAZ_00002713"/>
        <obo:IAO_0000115>Israel&apos;s fourth largest local council and largest Israeli Arab local council. It is located in the Lower Galilee in the North District, to the north of Nazareth and next to Sakhnin and Deir Hanna.</obo:IAO_0000115>
        <oboInOwl:hasOBONamespace>GAZ</oboInOwl:hasOBONamespace>
        <oboInOwl:id>GAZ:00078405</oboInOwl:id>
        <rdfs:label>Arraba Local Council</rdfs:label>
    </owl:NamedIndividual>
    


    <!-- http://purl.obolibrary.org/obo/GAZ_00078406 -->

    <owl:NamedIndividual rdf:about="http://purl.obolibrary.org/obo/GAZ_00078406">
        <obo:RO_0001025 rdf:resource="http://purl.obolibrary.org/obo/GAZ_00002713"/>
        <obo:IAO_0000115>An Israeli-Arab local council in Israel&apos;s North District, located in the Bet Netofa Valley.</obo:IAO_0000115>
        <oboInOwl:hasOBONamespace>GAZ</oboInOwl:hasOBONamespace>
        <oboInOwl:id>GAZ:00078406</oboInOwl:id>
        <rdfs:label>Eilabun Local Council</rdfs:label>
    </owl:NamedIndividual>
    


    <!-- http://purl.obolibrary.org/obo/GAZ_00078407 -->

    <owl:NamedIndividual rdf:about="http://purl.obolibrary.org/obo/GAZ_00078407">
        <obo:RO_0001025 rdf:resource="http://purl.obolibrary.org/obo/GAZ_00002713"/>
        <obo:IAO_0000115>An Arab local council in the Galilee region of northern Israel.</obo:IAO_0000115>
        <oboInOwl:hasOBONamespace>GAZ</oboInOwl:hasOBONamespace>
        <oboInOwl:id>GAZ:00078407</oboInOwl:id>
        <rdfs:label>Abu Sinan Local Council</rdfs:label>
    </owl:NamedIndividual>
    


    <!-- http://purl.obolibrary.org/obo/GAZ_00078408 -->

    <owl:NamedIndividual rdf:about="http://purl.obolibrary.org/obo/GAZ_00078408">
        <obo:RO_0001025 rdf:resource="http://purl.obolibrary.org/obo/GAZ_00002713"/>
        <obo:IAO_0000115>An Arab local council in the North District of Israel. It was declared as a local council in 1996.</obo:IAO_0000115>
        <oboInOwl:hasOBONamespace>GAZ</oboInOwl:hasOBONamespace>
        <oboInOwl:id>GAZ:00078408</oboInOwl:id>
        <rdfs:label>Ka&apos;abiyye-Tabbash-Hajajre Local Council</rdfs:label>
    </owl:NamedIndividual>
    


    <!-- http://purl.obolibrary.org/obo/GAZ_00078409 -->

    <owl:NamedIndividual rdf:about="http://purl.obolibrary.org/obo/GAZ_00078409">
        <obo:RO_0001025 rdf:resource="http://purl.obolibrary.org/obo/GAZ_00002713"/>
        <obo:IAO_0000115>A local council in the Northern District of Israel, south of the Lebanese border, on the northwestern slopes of Mount Meron.</obo:IAO_0000115>
        <oboInOwl:hasOBONamespace>GAZ</oboInOwl:hasOBONamespace>
        <oboInOwl:id>GAZ:00078409</oboInOwl:id>
        <rdfs:label>Fassuta Local Council</rdfs:label>
    </owl:NamedIndividual>
    


    <!-- http://purl.obolibrary.org/obo/GAZ_00078410 -->

    <owl:NamedIndividual rdf:about="http://purl.obolibrary.org/obo/GAZ_00078410">
        <obo:RO_0001025 rdf:resource="http://purl.obolibrary.org/obo/GAZ_00002713"/>
        <obo:IAO_0000115>An Arab local council in the North District of Israel, located about five km north of Nazareth. It was declared a local council in 1964.</obo:IAO_0000115>
        <oboInOwl:hasOBONamespace>GAZ</oboInOwl:hasOBONamespace>
        <oboInOwl:id>GAZ:00078410</oboInOwl:id>
        <rdfs:label>Ein Mahil Local Council</rdfs:label>
    </owl:NamedIndividual>
    


    <!-- http://purl.obolibrary.org/obo/GAZ_00078411 -->

    <owl:NamedIndividual rdf:about="http://purl.obolibrary.org/obo/GAZ_00078411">
        <obo:RO_0001025 rdf:resource="http://purl.obolibrary.org/obo/GAZ_00002713"/>
        <obo:IAO_0000115>An Alawite Local Council on the Hasbani River and on the border between Lebanon and Israeli-occupied Golan Heights.</obo:IAO_0000115>
        <oboInOwl:hasOBONamespace>GAZ</oboInOwl:hasOBONamespace>
        <oboInOwl:id>GAZ:00078411</oboInOwl:id>
        <rdfs:label>Ghajar Local Council</rdfs:label>
    </owl:NamedIndividual>
    


    <!-- http://purl.obolibrary.org/obo/GAZ_00078412 -->

    <owl:NamedIndividual rdf:about="http://purl.obolibrary.org/obo/GAZ_00078412">
        <obo:RO_0001025 rdf:resource="http://purl.obolibrary.org/obo/GAZ_00002713"/>
        <obo:IAO_0000115>An Israeli Arab local council on top of Mt. Meron, in Northern Israel.</obo:IAO_0000115>
        <oboInOwl:hasOBONamespace>GAZ</oboInOwl:hasOBONamespace>
        <oboInOwl:id>GAZ:00078412</oboInOwl:id>
        <rdfs:label>Beit Jann Local Council</rdfs:label>
    </owl:NamedIndividual>
    


    <!-- http://purl.obolibrary.org/obo/GAZ_00078413 -->

    <owl:NamedIndividual rdf:about="http://purl.obolibrary.org/obo/GAZ_00078413">
        <rdf:type rdf:resource="http://purl.obolibrary.org/obo/ENVO_00000856"/>
        <obo:RO_0001025 rdf:resource="http://purl.obolibrary.org/obo/GAZ_00002713"/>
        <obo:IAO_0000115>A Druze town in the northern Golan Heights, currently administered by Israel.</obo:IAO_0000115>
        <oboInOwl:hasOBONamespace>GAZ</oboInOwl:hasOBONamespace>
        <oboInOwl:id>GAZ:00078413</oboInOwl:id>
        <rdfs:label>Buq&apos;ata Local Council</rdfs:label>
    </owl:NamedIndividual>
    


    <!-- http://purl.obolibrary.org/obo/GAZ_00078414 -->

    <owl:NamedIndividual rdf:about="http://purl.obolibrary.org/obo/GAZ_00078414">
        <obo:RO_0001025 rdf:resource="http://purl.obolibrary.org/obo/GAZ_00002713"/>
        <obo:IAO_0000115>An Israeli-Arab local council in Israel&apos;s North District located 15km northwest of Nazareth.</obo:IAO_0000115>
        <oboInOwl:hasOBONamespace>GAZ</oboInOwl:hasOBONamespace>
        <oboInOwl:id>GAZ:00078414</oboInOwl:id>
        <rdfs:label>Bir al-Maksur Local Council</rdfs:label>
    </owl:NamedIndividual>
    


    <!-- http://purl.obolibrary.org/obo/GAZ_00078415 -->

    <owl:NamedIndividual rdf:about="http://purl.obolibrary.org/obo/GAZ_00078415">
        <obo:RO_0001025 rdf:resource="http://purl.obolibrary.org/obo/GAZ_00002713"/>
        <obo:IAO_0000115>A Moshava and a local council in the North District of Israel. Located south-west of Tiberias, it was declared a local council in 1951.</obo:IAO_0000115>
        <oboInOwl:hasOBONamespace>GAZ</oboInOwl:hasOBONamespace>
        <oboInOwl:id>GAZ:00078415</oboInOwl:id>
        <rdfs:label>Yavne&apos;el Local Council</rdfs:label>
    </owl:NamedIndividual>
    


    <!-- http://purl.obolibrary.org/obo/GAZ_00078416 -->

    <owl:NamedIndividual rdf:about="http://purl.obolibrary.org/obo/GAZ_00078416">
        <obo:RO_0001025 rdf:resource="http://purl.obolibrary.org/obo/GAZ_00002713"/>
        <obo:IAO_0000115>A Druze local council in the North District of Israel.</obo:IAO_0000115>
        <oboInOwl:hasOBONamespace>GAZ</oboInOwl:hasOBONamespace>
        <oboInOwl:id>GAZ:00078416</oboInOwl:id>
        <rdfs:label>Julis Local Council</rdfs:label>
    </owl:NamedIndividual>
    


    <!-- http://purl.obolibrary.org/obo/GAZ_00078417 -->

    <owl:NamedIndividual rdf:about="http://purl.obolibrary.org/obo/GAZ_00078417">
        <obo:RO_0001025 rdf:resource="http://purl.obolibrary.org/obo/GAZ_00002713"/>
        <obo:IAO_0000115>A Local Council located in the lower Galilee, Israel.</obo:IAO_0000115>
        <oboInOwl:hasOBONamespace>GAZ</oboInOwl:hasOBONamespace>
        <oboInOwl:id>GAZ:00078417</oboInOwl:id>
        <rdfs:label>Kfar Kama Local Council</rdfs:label>
    </owl:NamedIndividual>
    


    <!-- http://purl.obolibrary.org/obo/GAZ_00078418 -->

    <owl:NamedIndividual rdf:about="http://purl.obolibrary.org/obo/GAZ_00078418">
        <obo:RO_0001025 rdf:resource="http://purl.obolibrary.org/obo/GAZ_00002713"/>
        <obo:IAO_0000115>A Druze and Jewish Local Council in the northern part of the Golan Heights.</obo:IAO_0000115>
        <oboInOwl:hasOBONamespace>GAZ</oboInOwl:hasOBONamespace>
        <oboInOwl:id>GAZ:00078418</oboInOwl:id>
        <rdfs:label>Majdal Shams Local Council</rdfs:label>
    </owl:NamedIndividual>
    


    <!-- http://purl.obolibrary.org/obo/GAZ_00078419 -->

    <owl:NamedIndividual rdf:about="http://purl.obolibrary.org/obo/GAZ_00078419">
        <obo:RO_0001025 rdf:resource="http://purl.obolibrary.org/obo/GAZ_00002713"/>
        <obo:IAO_0000115>A Local Council in the Hula Valley, Northern District, Israel.</obo:IAO_0000115>
        <oboInOwl:hasOBONamespace>GAZ</oboInOwl:hasOBONamespace>
        <oboInOwl:id>GAZ:00078419</oboInOwl:id>
        <rdfs:label>Yesod HaMa&apos;ala Local Council</rdfs:label>
    </owl:NamedIndividual>
    


    <!-- http://purl.obolibrary.org/obo/GAZ_00078420 -->

    <owl:NamedIndividual rdf:about="http://purl.obolibrary.org/obo/GAZ_00078420">
        <obo:RO_0001025 rdf:resource="http://purl.obolibrary.org/obo/GAZ_00002713"/>
        <obo:IAO_0000115>A Local Council in the Golan Heights, Israel.</obo:IAO_0000115>
        <oboInOwl:hasOBONamespace>GAZ</oboInOwl:hasOBONamespace>
        <oboInOwl:id>GAZ:00078420</oboInOwl:id>
        <rdfs:label>Katzrin Local Council</rdfs:label>
    </owl:NamedIndividual>
    


    <!-- http://purl.obolibrary.org/obo/GAZ_00078421 -->

    <owl:NamedIndividual rdf:about="http://purl.obolibrary.org/obo/GAZ_00078421">
        <obo:RO_0001025 rdf:resource="http://purl.obolibrary.org/obo/GAZ_00002713"/>
        <obo:IAO_0000115>A multi-ethnic local council in Israel&apos;s North District.</obo:IAO_0000115>
        <oboInOwl:hasOBONamespace>GAZ</oboInOwl:hasOBONamespace>
        <oboInOwl:id>GAZ:00078421</oboInOwl:id>
        <rdfs:label>Maghar Local Council</rdfs:label>
    </owl:NamedIndividual>
    


    <!-- http://purl.obolibrary.org/obo/GAZ_00078422 -->

    <owl:NamedIndividual rdf:about="http://purl.obolibrary.org/obo/GAZ_00078422">
        <obo:RO_0001025 rdf:resource="http://purl.obolibrary.org/obo/GAZ_00002713"/>
        <obo:IAO_0000115>A Local Council in northern Israel. It is located in between Acre and Nahariyya on the Mediterranean coast.</obo:IAO_0000115>
        <oboInOwl:hasOBONamespace>GAZ</oboInOwl:hasOBONamespace>
        <oboInOwl:id>GAZ:00078422</oboInOwl:id>
        <rdfs:label>Mazra&apos;a Local Council</rdfs:label>
    </owl:NamedIndividual>
    


    <!-- http://purl.obolibrary.org/obo/GAZ_00078423 -->

    <owl:NamedIndividual rdf:about="http://purl.obolibrary.org/obo/GAZ_00078423">
        <obo:RO_0001025 rdf:resource="http://purl.obolibrary.org/obo/GAZ_00002713"/>
        <obo:IAO_0000115>An Israeli Druze local council in Israel&apos;s North District, northeast of Acre.</obo:IAO_0000115>
        <oboInOwl:hasOBONamespace>GAZ</oboInOwl:hasOBONamespace>
        <oboInOwl:id>GAZ:00078423</oboInOwl:id>
        <rdfs:label>Yirka Local Council</rdfs:label>
    </owl:NamedIndividual>
    


    <!-- http://purl.obolibrary.org/obo/GAZ_00078424 -->

    <owl:NamedIndividual rdf:about="http://purl.obolibrary.org/obo/GAZ_00078424">
        <obo:RO_0001025 rdf:resource="http://purl.obolibrary.org/obo/GAZ_00002713"/>
        <obo:IAO_0000115>A Local Council in the North District of Israel.</obo:IAO_0000115>
        <oboInOwl:hasOBONamespace>GAZ</oboInOwl:hasOBONamespace>
        <oboInOwl:id>GAZ:00078424</oboInOwl:id>
        <rdfs:label>Metula Local Council</rdfs:label>
    </owl:NamedIndividual>
    


    <!-- http://purl.obolibrary.org/obo/GAZ_00078425 -->

    <owl:NamedIndividual rdf:about="http://purl.obolibrary.org/obo/GAZ_00078425">
        <obo:RO_0001025 rdf:resource="http://purl.obolibrary.org/obo/GAZ_00002713"/>
        <obo:IAO_0000115>An Israeli-Arab Local Council located five km northeast of Nazareth in Israel&apos;s North District.</obo:IAO_0000115>
        <oboInOwl:hasOBONamespace>GAZ</oboInOwl:hasOBONamespace>
        <oboInOwl:id>GAZ:00078425</oboInOwl:id>
        <rdfs:label>Mashhad Local Council</rdfs:label>
    </owl:NamedIndividual>
    


    <!-- http://purl.obolibrary.org/obo/GAZ_00078426 -->

    <owl:NamedIndividual rdf:about="http://purl.obolibrary.org/obo/GAZ_00078426">
        <obo:RO_0001025 rdf:resource="http://purl.obolibrary.org/obo/GAZ_00002713"/>
        <obo:IAO_0000115>A Druze Local Council in the Golan Heights in the far north of Israel.</obo:IAO_0000115>
        <oboInOwl:hasOBONamespace>GAZ</oboInOwl:hasOBONamespace>
        <oboInOwl:id>GAZ:00078426</oboInOwl:id>
        <rdfs:label>Mas&apos;ada Local Council</rdfs:label>
    </owl:NamedIndividual>
    


    <!-- http://purl.obolibrary.org/obo/GAZ_00078427 -->

    <owl:NamedIndividual rdf:about="http://purl.obolibrary.org/obo/GAZ_00078427">
        <obo:RO_0001025 rdf:resource="http://purl.obolibrary.org/obo/GAZ_00002713"/>
        <obo:IAO_0000115>A Local Council in northern Israel, situated just south of Ma&apos;alot-Tarshiha and about 14 km south of the border with Lebanon.</obo:IAO_0000115>
        <oboInOwl:hasOBONamespace>GAZ</oboInOwl:hasOBONamespace>
        <oboInOwl:id>GAZ:00078427</oboInOwl:id>
        <rdfs:label>Kfar Vradim Local Council</rdfs:label>
    </owl:NamedIndividual>
    


    <!-- http://purl.obolibrary.org/obo/GAZ_00078428 -->

    <owl:NamedIndividual rdf:about="http://purl.obolibrary.org/obo/GAZ_00078428">
        <obo:RO_0001025 rdf:resource="http://purl.obolibrary.org/obo/GAZ_00002713"/>
        <obo:IAO_0000115>A local council in the North District of Israel, located on the side of the Haifa-Nazareth road about 4 km eastern to Kiryat Tivon. It was declared a local council in 1958.</obo:IAO_0000115>
        <oboInOwl:hasOBONamespace>GAZ</oboInOwl:hasOBONamespace>
        <oboInOwl:id>GAZ:00078428</oboInOwl:id>
        <rdfs:label>Ramat Yishai Local Council</rdfs:label>
    </owl:NamedIndividual>
    


    <!-- http://purl.obolibrary.org/obo/GAZ_00078429 -->

    <owl:NamedIndividual rdf:about="http://purl.obolibrary.org/obo/GAZ_00078429">
        <obo:RO_0001025 rdf:resource="http://purl.obolibrary.org/obo/GAZ_00002713"/>
        <obo:IAO_0000115>An Arab Local Council in the North District of Israel.</obo:IAO_0000115>
        <oboInOwl:hasOBONamespace>GAZ</oboInOwl:hasOBONamespace>
        <oboInOwl:id>GAZ:00078429</oboInOwl:id>
        <rdfs:label>Sha&apos;ab Local Council</rdfs:label>
    </owl:NamedIndividual>
    


    <!-- http://purl.obolibrary.org/obo/GAZ_00078430 -->

    <owl:NamedIndividual rdf:about="http://purl.obolibrary.org/obo/GAZ_00078430">
        <obo:RO_0001025 rdf:resource="http://purl.obolibrary.org/obo/GAZ_00002713"/>
        <obo:IAO_0000115>An Israeli-Arab Bedouin local council at the base of Mount Tabor in Israel&apos;s North District.</obo:IAO_0000115>
        <oboInOwl:hasOBONamespace>GAZ</oboInOwl:hasOBONamespace>
        <oboInOwl:id>GAZ:00078430</oboInOwl:id>
        <rdfs:label>Shibli-Umm al-Janam Local Council</rdfs:label>
    </owl:NamedIndividual>
    


    <!-- http://purl.obolibrary.org/obo/GAZ_00078431 -->

    <owl:NamedIndividual rdf:about="http://purl.obolibrary.org/obo/GAZ_00078431">
        <obo:RO_0001025 rdf:resource="http://purl.obolibrary.org/obo/GAZ_00002713"/>
        <obo:IAO_0000115>A Local Council in the Galilee region of northern Israel.</obo:IAO_0000115>
        <oboInOwl:hasOBONamespace>GAZ</oboInOwl:hasOBONamespace>
        <oboInOwl:id>GAZ:00078431</oboInOwl:id>
        <rdfs:label>Sajur Local Council</rdfs:label>
    </owl:NamedIndividual>
    


    <!-- http://purl.obolibrary.org/obo/GAZ_00078432 -->

    <owl:NamedIndividual rdf:about="http://purl.obolibrary.org/obo/GAZ_00078432">
        <obo:RO_0001025 rdf:resource="http://purl.obolibrary.org/obo/GAZ_00002713"/>
        <obo:IAO_0000115>An Arab local council in the North District of Israel. It was declared as a local council in 1990. Before a municipal merger in 1990, Yanuh-Jat was two villages: Yanuh and Jat.</obo:IAO_0000115>
        <oboInOwl:hasOBONamespace>GAZ</oboInOwl:hasOBONamespace>
        <oboInOwl:id>GAZ:00078432</oboInOwl:id>
        <rdfs:label>Yanuh-Jat Local Council</rdfs:label>
    </owl:NamedIndividual>
    


    <!-- http://purl.obolibrary.org/obo/GAZ_00078433 -->

    <owl:NamedIndividual rdf:about="http://purl.obolibrary.org/obo/GAZ_00078433">
        <obo:RO_0001025 rdf:resource="http://purl.obolibrary.org/obo/GAZ_00002713"/>
        <obo:IAO_0000115>A Bedouin Arab local council in the North District of Israel. It was formed by the merger of the two villages of Tuba and al-Zangariyye. It is 8.5 km east of Safed and 2 km west of the Golan Heights border with Israel.</obo:IAO_0000115>
        <oboInOwl:hasOBONamespace>GAZ</oboInOwl:hasOBONamespace>
        <oboInOwl:id>GAZ:00078433</oboInOwl:id>
        <rdfs:label>Tuba-Zangariyye Local Council</rdfs:label>
    </owl:NamedIndividual>
    


    <!-- http://purl.obolibrary.org/obo/GAZ_00078434 -->

    <owl:NamedIndividual rdf:about="http://purl.obolibrary.org/obo/GAZ_00078434">
        <obo:RO_0001025 rdf:resource="http://purl.obolibrary.org/obo/GAZ_00002713"/>
        <obo:IAO_0000115>An Israeli-Arab local council in the North District of Israel. It is located on Mount Tur&apos;an near the main road from Haifa to Tiberias, and about 7 km north of Nazareth.</obo:IAO_0000115>
        <oboInOwl:hasOBONamespace>GAZ</oboInOwl:hasOBONamespace>
        <oboInOwl:id>GAZ:00078434</oboInOwl:id>
        <rdfs:label>Tur&apos;an Local Council</rdfs:label>
    </owl:NamedIndividual>
    


    <!-- http://purl.obolibrary.org/obo/GAZ_00078435 -->

    <owl:NamedIndividual rdf:about="http://purl.obolibrary.org/obo/GAZ_00078435">
        <obo:RO_0001025 rdf:resource="http://purl.obolibrary.org/obo/GAZ_00002713"/>
        <obo:IAO_0000115>A Local Council located in the Upper Galilee on the eastern slopes of Mount Kna&apos;anin, the Northern District of Israel.</obo:IAO_0000115>
        <oboInOwl:hasOBONamespace>GAZ</oboInOwl:hasOBONamespace>
        <oboInOwl:id>GAZ:00078435</oboInOwl:id>
        <rdfs:label>Rosh Pinna Local Council</rdfs:label>
    </owl:NamedIndividual>
    


    <!-- http://purl.obolibrary.org/obo/GAZ_00078436 -->

    <owl:NamedIndividual rdf:about="http://purl.obolibrary.org/obo/GAZ_00078436">
        <obo:RO_0001025 rdf:resource="http://purl.obolibrary.org/obo/GAZ_00002713"/>
        <obo:IAO_0000115>An Arab local council located in the Lower Galilee, Israel. It forms part of the metropolitan area of Nazareth.</obo:IAO_0000115>
        <oboInOwl:hasOBONamespace>GAZ</oboInOwl:hasOBONamespace>
        <oboInOwl:id>GAZ:00078436</oboInOwl:id>
        <rdfs:label>Yafa an-Naseriyye Local Council</rdfs:label>
    </owl:NamedIndividual>
    


    <!-- http://purl.obolibrary.org/obo/GAZ_00078437 -->

    <owl:NamedIndividual rdf:about="http://purl.obolibrary.org/obo/GAZ_00078437">
        <obo:RO_0001025 rdf:resource="http://purl.obolibrary.org/obo/GAZ_00002713"/>
        <obo:IAO_0000115>A local council in the northern district of Israel. Established in 1910, and granted local council status in 1949.</obo:IAO_0000115>
        <oboInOwl:hasOBONamespace>GAZ</oboInOwl:hasOBONamespace>
        <oboInOwl:id>GAZ:00078437</oboInOwl:id>
        <rdfs:label>Migdal Local Council</rdfs:label>
    </owl:NamedIndividual>
    


    <!-- http://purl.obolibrary.org/obo/GAZ_00078438 -->

    <owl:NamedIndividual rdf:about="http://purl.obolibrary.org/obo/GAZ_00078438">
        <obo:RO_0001025 rdf:resource="http://purl.obolibrary.org/obo/GAZ_00002713"/>
        <obo:IAO_0000115>A local council in the North District of Israel.</obo:IAO_0000115>
        <oboInOwl:hasOBONamespace>GAZ</oboInOwl:hasOBONamespace>
        <oboInOwl:id>GAZ:00078438</oboInOwl:id>
        <rdfs:label>Rameh Local Council</rdfs:label>
    </owl:NamedIndividual>
    


    <!-- http://purl.obolibrary.org/obo/GAZ_00078439 -->

    <owl:NamedIndividual rdf:about="http://purl.obolibrary.org/obo/GAZ_00078439">
        <rdf:type rdf:resource="http://purl.obolibrary.org/obo/ENVO_00000856"/>
        <obo:RO_0001025 rdf:resource="http://purl.obolibrary.org/obo/GAZ_00002713"/>
        <obo:IAO_0000115>An Israeli Arab village in the Galilee, located between Nazareth and Qana of Galilee. The village attained Local council status in 1968.</obo:IAO_0000115>
        <oboInOwl:hasOBONamespace>GAZ</oboInOwl:hasOBONamespace>
        <oboInOwl:id>GAZ:00078439</oboInOwl:id>
        <rdfs:label>Reineh Local Council</rdfs:label>
    </owl:NamedIndividual>
    


    <!-- http://purl.obolibrary.org/obo/GAZ_00078440 -->

    <owl:NamedIndividual rdf:about="http://purl.obolibrary.org/obo/GAZ_00078440">
        <obo:RO_0001025 rdf:resource="http://purl.obolibrary.org/obo/GAZ_00002713"/>
        <obo:IAO_0000115>A local council in the Northern District of Israel located eight km east of Ma&apos;alot-Tarshiha in the Upper Galilee.</obo:IAO_0000115>
        <oboInOwl:hasOBONamespace>GAZ</oboInOwl:hasOBONamespace>
        <oboInOwl:id>GAZ:00078440</oboInOwl:id>
        <rdfs:label>Peki&apos;in Local Council</rdfs:label>
    </owl:NamedIndividual>
    


    <!-- http://purl.obolibrary.org/obo/GAZ_00078441 -->

    <owl:NamedIndividual rdf:about="http://purl.obolibrary.org/obo/GAZ_00078441">
        <obo:RO_0001025 rdf:resource="http://purl.obolibrary.org/obo/GAZ_00002713"/>
        <obo:IAO_0000115>An Arab local council in the North District Israel. It is located in the between the Lower and Upper Galilee, about 23 km east of Acre.</obo:IAO_0000115>
        <oboInOwl:hasOBONamespace>GAZ</oboInOwl:hasOBONamespace>
        <oboInOwl:id>GAZ:00078441</oboInOwl:id>
        <rdfs:label>Nahf Local Council</rdfs:label>
    </owl:NamedIndividual>
    


    <!-- http://purl.obolibrary.org/obo/GAZ_00078442 -->

    <owl:NamedIndividual rdf:about="http://purl.obolibrary.org/obo/GAZ_00078442">
        <obo:RO_0001025 rdf:resource="http://purl.obolibrary.org/obo/GAZ_00002712"/>
        <obo:IAO_0000115>A local council in the Benjamin region of the central West Bank, within the borders of the Matte Binyamin Regional Council. It is located in the hills north of Jerusalem just to the east of the Palestinian town of Al Bireh.</obo:IAO_0000115>
        <oboInOwl:hasOBONamespace>GAZ</oboInOwl:hasOBONamespace>
        <oboInOwl:id>GAZ:00078442</oboInOwl:id>
        <rdfs:label>Bet El Local Council</rdfs:label>
    </owl:NamedIndividual>
    


    <!-- http://purl.obolibrary.org/obo/GAZ_00078443 -->

    <owl:NamedIndividual rdf:about="http://purl.obolibrary.org/obo/GAZ_00078443">
        <obo:RO_0001025 rdf:resource="http://purl.obolibrary.org/obo/GAZ_00002712"/>
        <obo:IAO_0000115>A local council in Samaria, West Bank.</obo:IAO_0000115>
        <oboInOwl:hasOBONamespace>GAZ</oboInOwl:hasOBONamespace>
        <oboInOwl:id>GAZ:00078443</oboInOwl:id>
        <rdfs:label>Immanuel Local Council</rdfs:label>
    </owl:NamedIndividual>
    


    <!-- http://purl.obolibrary.org/obo/GAZ_00078444 -->

    <owl:NamedIndividual rdf:about="http://purl.obolibrary.org/obo/GAZ_00078444">
        <obo:RO_0001025 rdf:resource="http://purl.obolibrary.org/obo/GAZ_00002712"/>
        <obo:IAO_0000115>An Israeli Local Council located in the seam zone on the western edge of Samaria in the central West Bank. It was granted local council status in 1987.</obo:IAO_0000115>
        <oboInOwl:hasOBONamespace>GAZ</oboInOwl:hasOBONamespace>
        <oboInOwl:id>GAZ:00078444</oboInOwl:id>
        <rdfs:label>Alfei Menashe Local Council</rdfs:label>
    </owl:NamedIndividual>
    


    <!-- http://purl.obolibrary.org/obo/GAZ_00078445 -->

    <owl:NamedIndividual rdf:about="http://purl.obolibrary.org/obo/GAZ_00078445">
        <obo:RO_0001025 rdf:resource="http://purl.obolibrary.org/obo/GAZ_00002712"/>
        <obo:IAO_0000115>A local council, located northwest of Jerusalem. While it lies within the borders of the Matte Binyamin Regional Council, it is a separate municipal entity.</obo:IAO_0000115>
        <oboInOwl:hasOBONamespace>GAZ</oboInOwl:hasOBONamespace>
        <oboInOwl:id>GAZ:00078445</oboInOwl:id>
        <rdfs:label>Giv&apos;at Ze&apos;ev Local Council</rdfs:label>
    </owl:NamedIndividual>
    


    <!-- http://purl.obolibrary.org/obo/GAZ_00078446 -->

    <owl:NamedIndividual rdf:about="http://purl.obolibrary.org/obo/GAZ_00078446">
        <obo:RO_0001025 rdf:resource="http://purl.obolibrary.org/obo/GAZ_00002712"/>
        <obo:IAO_0000115>A Local Council in Judea and Samaria Area.</obo:IAO_0000115>
        <oboInOwl:hasOBONamespace>GAZ</oboInOwl:hasOBONamespace>
        <oboInOwl:id>GAZ:00078446</oboInOwl:id>
        <rdfs:label>Beit Arieh Local Council</rdfs:label>
    </owl:NamedIndividual>
    


    <!-- http://purl.obolibrary.org/obo/GAZ_00078447 -->

    <owl:NamedIndividual rdf:about="http://purl.obolibrary.org/obo/GAZ_00078447">
        <obo:RO_0001025 rdf:resource="http://purl.obolibrary.org/obo/GAZ_00002712"/>
        <obo:IAO_0000115>A Local Council in Judea (southern West Bank), located south of Jerusalem, between the cities of Bethlehem and Hebron. Efrat was established in 1980.</obo:IAO_0000115>
        <oboInOwl:hasOBONamespace>GAZ</oboInOwl:hasOBONamespace>
        <oboInOwl:id>GAZ:00078447</oboInOwl:id>
        <rdfs:label>Efrat Local Council</rdfs:label>
    </owl:NamedIndividual>
    


    <!-- http://purl.obolibrary.org/obo/GAZ_00078448 -->

    <owl:NamedIndividual rdf:about="http://purl.obolibrary.org/obo/GAZ_00078448">
        <obo:RO_0001025 rdf:resource="http://purl.obolibrary.org/obo/GAZ_00002712"/>
        <obo:IAO_0000115>A regional council in the Jordan River Valley of the West Bank. The municipal territory of the council reaches from Mehola in the north, near the Beit She&apos;an valley, to Jericho in the south, and includes over twenty Israeli settlements.</obo:IAO_0000115>
        <oboInOwl:hasOBONamespace>GAZ</oboInOwl:hasOBONamespace>
        <oboInOwl:id>GAZ:00078448</oboInOwl:id>
        <rdfs:label>Biq&apos;at HaYarden Regional Council</rdfs:label>
    </owl:NamedIndividual>
    


    <!-- http://purl.obolibrary.org/obo/GAZ_00078449 -->

    <owl:NamedIndividual rdf:about="http://purl.obolibrary.org/obo/GAZ_00078449">
        <obo:RO_0001025 rdf:resource="http://purl.obolibrary.org/obo/GAZ_00002712"/>
        <obo:IAO_0000115>A Local Council in Judea and Samaria Area.</obo:IAO_0000115>
        <oboInOwl:hasOBONamespace>GAZ</oboInOwl:hasOBONamespace>
        <oboInOwl:id>GAZ:00078449</oboInOwl:id>
        <rdfs:label>Har Adar Local Council</rdfs:label>
    </owl:NamedIndividual>
    


    <!-- http://purl.obolibrary.org/obo/GAZ_00078450 -->

    <owl:NamedIndividual rdf:about="http://purl.obolibrary.org/obo/GAZ_00078450">
        <obo:RO_0001025 rdf:resource="http://purl.obolibrary.org/obo/GAZ_00002712"/>
        <obo:IAO_0000115>A city on the West Bank. It is situated approximately 40 km east of Tel Aviv, 40 km west of the Jordan River, and 60 km northwest of Jerusalem. It lies southwest of Nablus/Shechem, north of Ramallah and southeast of Qalqilyah.</obo:IAO_0000115>
        <oboInOwl:hasOBONamespace>GAZ</oboInOwl:hasOBONamespace>
        <oboInOwl:id>GAZ:00078450</oboInOwl:id>
        <rdfs:label>City of Ariel</rdfs:label>
    </owl:NamedIndividual>
    


    <!-- http://purl.obolibrary.org/obo/GAZ_00078451 -->

    <owl:NamedIndividual rdf:about="http://purl.obolibrary.org/obo/GAZ_00078451">
        <obo:RO_0001025 rdf:resource="http://purl.obolibrary.org/obo/GAZ_00002712"/>
        <obo:IAO_0000115>A Local Council in Judea and Samaria Area.</obo:IAO_0000115>
        <oboInOwl:hasOBONamespace>GAZ</oboInOwl:hasOBONamespace>
        <oboInOwl:id>GAZ:00078451</oboInOwl:id>
        <rdfs:label>Oranit Local Council</rdfs:label>
    </owl:NamedIndividual>
    


    <!-- http://purl.obolibrary.org/obo/GAZ_00078452 -->

    <owl:NamedIndividual rdf:about="http://purl.obolibrary.org/obo/GAZ_00078452">
        <rdf:type rdf:resource="http://purl.obolibrary.org/obo/ENVO_00000062"/>
        <obo:RO_0001025 rdf:resource="http://purl.obolibrary.org/obo/GAZ_00002712"/>
        <obo:IAO_0000115>An Israeli settlement and city in the foothills of the Judean Mountains of central Israel, midway between Jerusalem and Tel Aviv.</obo:IAO_0000115>
        <oboInOwl:hasOBONamespace>GAZ</oboInOwl:hasOBONamespace>
        <oboInOwl:id>GAZ:00078452</oboInOwl:id>
        <rdfs:label>City of Modi&apos;in Illit</rdfs:label>
    </owl:NamedIndividual>
    


    <!-- http://purl.obolibrary.org/obo/GAZ_00078453 -->

    <owl:NamedIndividual rdf:about="http://purl.obolibrary.org/obo/GAZ_00078453">
        <obo:RO_0001025 rdf:resource="http://purl.obolibrary.org/obo/GAZ_00002712"/>
        <obo:IAO_0000115>A regional council in the southern Samarian hills, or rather, the southern part of the northern area of the West Bank. The seat of the council is Psagot.</obo:IAO_0000115>
        <oboInOwl:hasOBONamespace>GAZ</oboInOwl:hasOBONamespace>
        <oboInOwl:id>GAZ:00078453</oboInOwl:id>
        <rdfs:label>Matte Binyamin Regional Council</rdfs:label>
    </owl:NamedIndividual>
    


    <!-- http://purl.obolibrary.org/obo/GAZ_00078454 -->

    <owl:NamedIndividual rdf:about="http://purl.obolibrary.org/obo/GAZ_00078454">
        <obo:RO_0001025 rdf:resource="http://purl.obolibrary.org/obo/GAZ_00002712"/>
        <obo:IAO_0000115>A regional council in the northern Judean hills, or rather, the northern part of the southern area of the West Bank, administering the settlements in the Gush Etzion region, as well as others nearby.</obo:IAO_0000115>
        <oboInOwl:hasOBONamespace>GAZ</oboInOwl:hasOBONamespace>
        <oboInOwl:id>GAZ:00078454</oboInOwl:id>
        <rdfs:label>Gush Etzion Regional Council</rdfs:label>
    </owl:NamedIndividual>
    


    <!-- http://purl.obolibrary.org/obo/GAZ_00078455 -->

    <owl:NamedIndividual rdf:about="http://purl.obolibrary.org/obo/GAZ_00078455">
        <obo:RO_0001025 rdf:resource="http://purl.obolibrary.org/obo/GAZ_00002712"/>
        <obo:IAO_0000115>A regional council in the Judean desert near the western shores of the Dead Sea in Israel.</obo:IAO_0000115>
        <oboInOwl:hasOBONamespace>GAZ</oboInOwl:hasOBONamespace>
        <oboInOwl:id>GAZ:00078455</oboInOwl:id>
        <rdfs:label>Megilot Dead Sea Regional Council</rdfs:label>
    </owl:NamedIndividual>
    


    <!-- http://purl.obolibrary.org/obo/GAZ_00078456 -->

    <owl:NamedIndividual rdf:about="http://purl.obolibrary.org/obo/GAZ_00078456">
        <obo:RO_0001025 rdf:resource="http://purl.obolibrary.org/obo/GAZ_00002712"/>
        <obo:IAO_0000115>An Israeli regional council in the southern Judean Hills are of Mount Hebron in the southern part of the West Bank, administering settlements in the Hebron region, as well as others nearby.</obo:IAO_0000115>
        <oboInOwl:hasOBONamespace>GAZ</oboInOwl:hasOBONamespace>
        <oboInOwl:id>GAZ:00078456</oboInOwl:id>
        <rdfs:label>Har Hebron Regional Council</rdfs:label>
    </owl:NamedIndividual>
    


    <!-- http://purl.obolibrary.org/obo/GAZ_00078457 -->

    <owl:NamedIndividual rdf:about="http://purl.obolibrary.org/obo/GAZ_00078457">
        <obo:RO_0001025 rdf:resource="http://purl.obolibrary.org/obo/GAZ_00002712"/>
        <obo:IAO_0000115>A regional council in the northern Samarian hills, also known as the northern part of the northern half of the West Bank.</obo:IAO_0000115>
        <oboInOwl:hasOBONamespace>GAZ</oboInOwl:hasOBONamespace>
        <oboInOwl:id>GAZ:00078457</oboInOwl:id>
        <rdfs:label>Shomron Regional Council</rdfs:label>
    </owl:NamedIndividual>
    


    <!-- http://purl.obolibrary.org/obo/GAZ_00078458 -->

    <owl:NamedIndividual rdf:about="http://purl.obolibrary.org/obo/GAZ_00078458">
        <obo:RO_0001025 rdf:resource="http://purl.obolibrary.org/obo/GAZ_00002712"/>
        <obo:IAO_0000115>An Israeli Local Council located in the northern West Bank/Samaria.</obo:IAO_0000115>
        <oboInOwl:hasOBONamespace>GAZ</oboInOwl:hasOBONamespace>
        <oboInOwl:id>GAZ:00078458</oboInOwl:id>
        <rdfs:label>Kedumim Local Council</rdfs:label>
    </owl:NamedIndividual>
    


    <!-- http://purl.obolibrary.org/obo/GAZ_00078459 -->

    <owl:NamedIndividual rdf:about="http://purl.obolibrary.org/obo/GAZ_00078459">
        <obo:RO_0001025 rdf:resource="http://purl.obolibrary.org/obo/GAZ_00002712"/>
        <obo:IAO_0000115>An Israeli local council located along the eastern slopes of the Samarian mountains in the Jordan Valley, within the West Bank. Founded in 1978.</obo:IAO_0000115>
        <oboInOwl:hasOBONamespace>GAZ</oboInOwl:hasOBONamespace>
        <oboInOwl:id>GAZ:00078459</oboInOwl:id>
        <rdfs:label>Ma&apos;ale Efraim Local Council</rdfs:label>
    </owl:NamedIndividual>
    


    <!-- http://purl.obolibrary.org/obo/GAZ_00078460 -->

    <owl:NamedIndividual rdf:about="http://purl.obolibrary.org/obo/GAZ_00078460">
        <obo:RO_0001025 rdf:resource="http://purl.obolibrary.org/obo/GAZ_00002712"/>
        <obo:IAO_0000115>An Israeli local council that was first established in 1977. in the western Samaria region (West Bank), east of Kfar Saba. It is 48 km north-east of Tel Aviv and 85 km north of Jerusalem.</obo:IAO_0000115>
        <oboInOwl:hasOBONamespace>GAZ</oboInOwl:hasOBONamespace>
        <oboInOwl:id>GAZ:00078460</oboInOwl:id>
        <rdfs:label>Karnei Shomron Local Council</rdfs:label>
    </owl:NamedIndividual>
    


    <!-- http://purl.obolibrary.org/obo/GAZ_00078461 -->

    <owl:NamedIndividual rdf:about="http://purl.obolibrary.org/obo/GAZ_00078461">
        <obo:RO_0001025 rdf:resource="http://purl.obolibrary.org/obo/GAZ_00002712"/>
        <obo:IAO_0000115>A local council in the Western Samarian region of the West Bank. Established in 1977.</obo:IAO_0000115>
        <oboInOwl:hasOBONamespace>GAZ</oboInOwl:hasOBONamespace>
        <oboInOwl:id>GAZ:00078461</oboInOwl:id>
        <rdfs:label>Elkana Local Council</rdfs:label>
    </owl:NamedIndividual>
    


    <!-- http://purl.obolibrary.org/obo/GAZ_00078462 -->

    <owl:NamedIndividual rdf:about="http://purl.obolibrary.org/obo/GAZ_00078462">
        <obo:RO_0001025 rdf:resource="http://purl.obolibrary.org/obo/GAZ_00002712"/>
        <obo:IAO_0000115>An urban Jewish Local Council in Southern Judea (Southern West Bank) adjoining the city of Hebron.</obo:IAO_0000115>
        <oboInOwl:hasOBONamespace>GAZ</oboInOwl:hasOBONamespace>
        <oboInOwl:id>GAZ:00078462</oboInOwl:id>
        <rdfs:label>Kiryat Arba Local Council</rdfs:label>
    </owl:NamedIndividual>
    


    <!-- http://purl.obolibrary.org/obo/GAZ_00078463 -->

    <owl:NamedIndividual rdf:about="http://purl.obolibrary.org/obo/GAZ_00078463">
        <rdf:type rdf:resource="http://purl.obolibrary.org/obo/ENVO_00000062"/>
        <obo:RO_0001025 rdf:resource="http://purl.obolibrary.org/obo/GAZ_00002712"/>
        <obo:IAO_0000115>An Israeli settlement and city west of Gush Etzion in the northern Judea region of the West Bank.</obo:IAO_0000115>
        <oboInOwl:hasOBONamespace>GAZ</oboInOwl:hasOBONamespace>
        <oboInOwl:id>GAZ:00078463</oboInOwl:id>
        <rdfs:label>City of Betar Illit</rdfs:label>
    </owl:NamedIndividual>
    


    <!-- http://purl.obolibrary.org/obo/GAZ_00078464 -->

    <owl:NamedIndividual rdf:about="http://purl.obolibrary.org/obo/GAZ_00078464">
        <obo:RO_0001025 rdf:resource="http://purl.obolibrary.org/obo/GAZ_00002712"/>
        <obo:IAO_0000115>An Israeli Settlement and city located east of Jerusalem in the West Bank and on the edge of the Judean desert. It is located within the boundaries of the Gush Etzion Regional Council, but has had its own mayor and municipality independent of the council&apos;s jurisdiction since achieving city status in 1991.</obo:IAO_0000115>
        <oboInOwl:hasOBONamespace>GAZ</oboInOwl:hasOBONamespace>
        <oboInOwl:id>GAZ:00078464</oboInOwl:id>
        <rdfs:label>City of Ma&apos;ale Adummim</rdfs:label>
    </owl:NamedIndividual>
    


    <!-- http://purl.obolibrary.org/obo/GAZ_00089761 -->

    <owl:NamedIndividual rdf:about="http://purl.obolibrary.org/obo/GAZ_00089761">
        <obo:RO_0001025 rdf:resource="http://purl.obolibrary.org/obo/GAZ_00000669"/>
        <obo:IAO_0000115>A wetland protected area. Established 1985.</obo:IAO_0000115>
        <oboInOwl:hasOBONamespace>GAZ</oboInOwl:hasOBONamespace>
        <oboInOwl:id>GAZ:00089761</oboInOwl:id>
        <rdfs:label>Zaranik Protected Area</rdfs:label>
    </owl:NamedIndividual>
    


    <!-- http://purl.obolibrary.org/obo/GAZ_00089762 -->

    <owl:NamedIndividual rdf:about="http://purl.obolibrary.org/obo/GAZ_00089762">
        <obo:RO_0001025 rdf:resource="http://purl.obolibrary.org/obo/GAZ_00000670"/>
        <obo:IAO_0000115>A protected area located at the meeting point of the Gulf of Suez and Aqaba Gulf. The Eastern border of Ras Mohamed Protected Area is a rocky wall with the gulf water where there are coral reefs. There is also the Mangrove channel which separates Ras Mohamed Peninsula from Elbayra Island at a length of approximately 250 m. Establishd 1983.</obo:IAO_0000115>
        <oboInOwl:hasOBONamespace>GAZ</oboInOwl:hasOBONamespace>
        <oboInOwl:id>GAZ:00089762</oboInOwl:id>
        <rdfs:label>Ras Mohamed Protected Area</rdfs:label>
    </owl:NamedIndividual>
    


    <!-- http://purl.obolibrary.org/obo/GAZ_00089763 -->

    <owl:NamedIndividual rdf:about="http://purl.obolibrary.org/obo/GAZ_00089763">
        <obo:RO_0001025 rdf:resource="http://purl.obolibrary.org/obo/GAZ_00000669"/>
        <obo:IAO_0000115>A protected area of coastal marshes. Established in 1985.</obo:IAO_0000115>
        <oboInOwl:hasOBONamespace>GAZ</oboInOwl:hasOBONamespace>
        <oboInOwl:id>GAZ:00089763</oboInOwl:id>
        <rdfs:label>Ahrash Protectorate</rdfs:label>
    </owl:NamedIndividual>
    


    <!-- http://purl.obolibrary.org/obo/GAZ_00089778 -->

    <owl:NamedIndividual rdf:about="http://purl.obolibrary.org/obo/GAZ_00089778">
        <obo:RO_0001025 rdf:resource="http://purl.obolibrary.org/obo/GAZ_00000670"/>
        <obo:IAO_0000115>A protected area established in 1992.</obo:IAO_0000115>
        <oboInOwl:hasOBONamespace>GAZ</oboInOwl:hasOBONamespace>
        <oboInOwl:id>GAZ:00089778</oboInOwl:id>
        <rdfs:label>Nabaq Protectorate</rdfs:label>
    </owl:NamedIndividual>
    


    <!-- http://purl.obolibrary.org/obo/GAZ_00089779 -->

    <owl:NamedIndividual rdf:about="http://purl.obolibrary.org/obo/GAZ_00089779">
        <obo:RO_0001025 rdf:resource="http://purl.obolibrary.org/obo/GAZ_00000670"/>
        <obo:IAO_0000115>A protected area established in 1992.</obo:IAO_0000115>
        <oboInOwl:hasOBONamespace>GAZ</oboInOwl:hasOBONamespace>
        <oboInOwl:id>GAZ:00089779</oboInOwl:id>
        <rdfs:label>Abu Galum Protectorate</rdfs:label>
    </owl:NamedIndividual>
    


    <!-- http://purl.obolibrary.org/obo/GAZ_00089780 -->

    <owl:NamedIndividual rdf:about="http://purl.obolibrary.org/obo/GAZ_00089780">
        <obo:RO_0001025 rdf:resource="http://purl.obolibrary.org/obo/GAZ_00000670"/>
        <obo:IAO_0000115>A protected area established in 1998.</obo:IAO_0000115>
        <oboInOwl:hasOBONamespace>GAZ</oboInOwl:hasOBONamespace>
        <oboInOwl:id>GAZ:00089780</oboInOwl:id>
        <rdfs:label>Taba Protectorate</rdfs:label>
    </owl:NamedIndividual>
    


    <!-- http://purl.obolibrary.org/obo/GAZ_00176005 -->

    <owl:NamedIndividual rdf:about="http://purl.obolibrary.org/obo/GAZ_00176005">
        <obo:RO_0001025 rdf:resource="http://purl.obolibrary.org/obo/GAZ_00000670"/>
        <obo:RO_0001025 rdf:resource="http://purl.obolibrary.org/obo/GAZ_00007862"/>
        <obo:IAO_0000115>An island in the northern Gulf of Aqaba off the shore of Egypt&apos;s eastern Sinai Peninsula.</obo:IAO_0000115>
        <oboInOwl:hasOBONamespace>GAZ</oboInOwl:hasOBONamespace>
        <oboInOwl:id>GAZ:00176005</oboInOwl:id>
        <rdfs:label>Pharaoh&apos;s Island</rdfs:label>
    </owl:NamedIndividual>
    


    <!-- http://purl.obolibrary.org/obo/GAZ_00193785 -->

    <owl:NamedIndividual rdf:about="http://purl.obolibrary.org/obo/GAZ_00193785">
        <obo:RO_0001025 rdf:resource="http://purl.obolibrary.org/obo/GAZ_00007520"/>
        <obo:IAO_0000115>A river. A tributary of the Jordan River.</obo:IAO_0000115>
        <oboInOwl:hasOBONamespace>GAZ</oboInOwl:hasOBONamespace>
        <oboInOwl:id>GAZ:00193785</oboInOwl:id>
        <rdfs:label>Banias River</rdfs:label>
    </owl:NamedIndividual>
    


    <!-- http://purl.obolibrary.org/obo/GAZ_00193791 -->

    <owl:NamedIndividual rdf:about="http://purl.obolibrary.org/obo/GAZ_00193791">
        <obo:IAO_0000115>The lowest nature reserve in the world, with a spectacular array of scenery near the east cost of the Dead Sea. The reserve is located within the deep Wadi Mujib gorge, which enters the Dead Sea at 410 m below sea level. The Reserve extends to the Kerak and Madaba mountains to the north and south.</obo:IAO_0000115>
        <oboInOwl:hasOBONamespace>GAZ</oboInOwl:hasOBONamespace>
        <oboInOwl:id>GAZ:00193791</oboInOwl:id>
        <rdfs:label>Mujib Nature Reserve</rdfs:label>
    </owl:NamedIndividual>
    


    <!-- http://purl.obolibrary.org/obo/GAZ_00193799 -->

    <owl:NamedIndividual rdf:about="http://purl.obolibrary.org/obo/GAZ_00193799">
        <obo:RO_0001025 rdf:resource="http://purl.obolibrary.org/obo/GAZ_00057704"/>
        <obo:IAO_0000115>A geological erosional landform of Israel&apos;s Negev desert.</obo:IAO_0000115>
        <oboInOwl:hasOBONamespace>GAZ</oboInOwl:hasOBONamespace>
        <oboInOwl:id>GAZ:00193799</oboInOwl:id>
        <rdfs:label>Makhtesh Katan</rdfs:label>
    </owl:NamedIndividual>
    


    <!-- http://purl.obolibrary.org/obo/GAZ_00193800 -->

    <owl:NamedIndividual rdf:about="http://purl.obolibrary.org/obo/GAZ_00193800">
        <obo:RO_0001025 rdf:resource="http://purl.obolibrary.org/obo/GAZ_00193802"/>
        <obo:IAO_0000115>A geological erosional landform of Israel&apos;s Negev desert. Located at the peak of Mount Negev, some 85 km south of the city of Beersheba.</obo:IAO_0000115>
        <oboInOwl:hasOBONamespace>GAZ</oboInOwl:hasOBONamespace>
        <oboInOwl:id>GAZ:00193800</oboInOwl:id>
        <rdfs:label>Makhtesh Ramon</rdfs:label>
    </owl:NamedIndividual>
    


    <!-- http://purl.obolibrary.org/obo/GAZ_00193801 -->

    <owl:NamedIndividual rdf:about="http://purl.obolibrary.org/obo/GAZ_00193801">
        <obo:RO_0001025 rdf:resource="http://purl.obolibrary.org/obo/GAZ_00057704"/>
        <obo:IAO_0000115>A geological erosional landform of Israel&apos;s Negev desert. It is drained by two rivers, the Nahal Ramon and Nahal Ardon.</obo:IAO_0000115>
        <oboInOwl:hasOBONamespace>GAZ</oboInOwl:hasOBONamespace>
        <oboInOwl:id>GAZ:00193801</oboInOwl:id>
        <rdfs:label>Makhtesh Gadol</rdfs:label>
    </owl:NamedIndividual>
    


    <!-- http://purl.obolibrary.org/obo/GAZ_00193802 -->

    <owl:NamedIndividual rdf:about="http://purl.obolibrary.org/obo/GAZ_00193802">
        <obo:RO_0001025 rdf:resource="http://purl.obolibrary.org/obo/GAZ_00057704"/>
        <obo:IAO_0000115>A protected area.</obo:IAO_0000115>
        <oboInOwl:hasOBONamespace>GAZ</oboInOwl:hasOBONamespace>
        <oboInOwl:id>GAZ:00193802</oboInOwl:id>
        <rdfs:label>Makhtesh Ramon, Visitors Center, Hai Ramon, Geological and Archaeological Park</rdfs:label>
    </owl:NamedIndividual>
    


    <!-- http://purl.obolibrary.org/obo/GAZ_00193803 -->

    <owl:NamedIndividual rdf:about="http://purl.obolibrary.org/obo/GAZ_00193803">
        <obo:RO_0001025 rdf:resource="http://purl.obolibrary.org/obo/GAZ_00057704"/>
        <obo:IAO_0000115>A protected area. An archeological site.</obo:IAO_0000115>
        <oboInOwl:hasOBONamespace>GAZ</oboInOwl:hasOBONamespace>
        <oboInOwl:id>GAZ:00193803</oboInOwl:id>
        <rdfs:label>Avdat National Park</rdfs:label>
    </owl:NamedIndividual>
    


    <!-- http://purl.obolibrary.org/obo/GAZ_00193804 -->

    <owl:NamedIndividual rdf:about="http://purl.obolibrary.org/obo/GAZ_00193804">
        <obo:RO_0001025 rdf:resource="http://purl.obolibrary.org/obo/GAZ_00007862"/>
        <obo:IAO_0000115>A protected area located on the Red Sea south of Eilat.</obo:IAO_0000115>
        <oboInOwl:hasOBONamespace>GAZ</oboInOwl:hasOBONamespace>
        <oboInOwl:id>GAZ:00193804</oboInOwl:id>
        <rdfs:label>Coral Beach Nature Reserve</rdfs:label>
    </owl:NamedIndividual>
    


    <!-- http://purl.obolibrary.org/obo/GAZ_00193805 -->

    <owl:NamedIndividual rdf:about="http://purl.obolibrary.org/obo/GAZ_00193805">
        <obo:RO_0001025 rdf:resource="http://purl.obolibrary.org/obo/GAZ_00193825"/>
        <obo:IAO_0000115>A protected area.</obo:IAO_0000115>
        <oboInOwl:hasOBONamespace>GAZ</oboInOwl:hasOBONamespace>
        <oboInOwl:id>GAZ:00193805</oboInOwl:id>
        <rdfs:label>En Avdat National Park</rdfs:label>
    </owl:NamedIndividual>
    


    <!-- http://purl.obolibrary.org/obo/GAZ_00193806 -->

    <owl:NamedIndividual rdf:about="http://purl.obolibrary.org/obo/GAZ_00193806">
        <obo:RO_0001025 rdf:resource="http://purl.obolibrary.org/obo/GAZ_00193805"/>
        <obo:IAO_0000115>A spring.</obo:IAO_0000115>
        <oboInOwl:hasOBONamespace>GAZ</oboInOwl:hasOBONamespace>
        <oboInOwl:id>GAZ:00193806</oboInOwl:id>
        <rdfs:label>En Avdat</rdfs:label>
    </owl:NamedIndividual>
    


    <!-- http://purl.obolibrary.org/obo/GAZ_00193807 -->

    <owl:NamedIndividual rdf:about="http://purl.obolibrary.org/obo/GAZ_00193807">
        <obo:RO_0001025 rdf:resource="http://purl.obolibrary.org/obo/GAZ_00057704"/>
        <obo:IAO_0000115>A protected area located near the northwestern Negev town of Ofakim.</obo:IAO_0000115>
        <oboInOwl:hasOBONamespace>GAZ</oboInOwl:hasOBONamespace>
        <oboInOwl:id>GAZ:00193807</oboInOwl:id>
        <rdfs:label>Eshkol National Park</rdfs:label>
    </owl:NamedIndividual>
    


    <!-- http://purl.obolibrary.org/obo/GAZ_00193808 -->

    <owl:NamedIndividual rdf:about="http://purl.obolibrary.org/obo/GAZ_00193808">
        <obo:RO_0001025 rdf:resource="http://purl.obolibrary.org/obo/GAZ_00057704"/>
        <obo:IAO_0000115>A protected area located near the modern town of Dimona. An archeological site.</obo:IAO_0000115>
        <oboInOwl:hasOBONamespace>GAZ</oboInOwl:hasOBONamespace>
        <oboInOwl:id>GAZ:00193808</oboInOwl:id>
        <rdfs:label>Mamshit National Park</rdfs:label>
    </owl:NamedIndividual>
    


    <!-- http://purl.obolibrary.org/obo/GAZ_00193809 -->

    <owl:NamedIndividual rdf:about="http://purl.obolibrary.org/obo/GAZ_00193809">
        <obo:RO_0001025 rdf:resource="http://purl.obolibrary.org/obo/GAZ_00057704"/>
        <obo:IAO_0000115>A protected area located in the western Negev not far from the Egyptian border at Nitsana. An archeological site.</obo:IAO_0000115>
        <oboInOwl:hasOBONamespace>GAZ</oboInOwl:hasOBONamespace>
        <oboInOwl:id>GAZ:00193809</oboInOwl:id>
        <rdfs:label>Shivta National Park</rdfs:label>
    </owl:NamedIndividual>
    


    <!-- http://purl.obolibrary.org/obo/GAZ_00193810 -->

    <owl:NamedIndividual rdf:about="http://purl.obolibrary.org/obo/GAZ_00193810">
        <obo:RO_0001025 rdf:resource="http://purl.obolibrary.org/obo/GAZ_00057704"/>
        <obo:IAO_0000115>A protected area northwest of the modern city of Arad in the northern Negev. An archeological site.</obo:IAO_0000115>
        <oboInOwl:hasOBONamespace>GAZ</oboInOwl:hasOBONamespace>
        <oboInOwl:id>GAZ:00193810</oboInOwl:id>
        <rdfs:label>Tel Arad National Park</rdfs:label>
    </owl:NamedIndividual>
    


    <!-- http://purl.obolibrary.org/obo/GAZ_00193811 -->

    <owl:NamedIndividual rdf:about="http://purl.obolibrary.org/obo/GAZ_00193811">
        <obo:RO_0001025 rdf:resource="http://purl.obolibrary.org/obo/GAZ_00057704"/>
        <obo:IAO_0000115>A protected area. An archeological site.</obo:IAO_0000115>
        <oboInOwl:hasOBONamespace>GAZ</oboInOwl:hasOBONamespace>
        <oboInOwl:id>GAZ:00193811</oboInOwl:id>
        <rdfs:label>Tel Be&apos;er Sheva National Park</rdfs:label>
    </owl:NamedIndividual>
    


    <!-- http://purl.obolibrary.org/obo/GAZ_00193812 -->

    <owl:NamedIndividual rdf:about="http://purl.obolibrary.org/obo/GAZ_00193812">
        <obo:RO_0001025 rdf:resource="http://purl.obolibrary.org/obo/GAZ_00057704"/>
        <obo:IAO_0000115>A breeding and reacclimation center administered by the Israel Nature Reserves &amp; National Parks Authority, situated in the Southern Arabah near Yotvata.</obo:IAO_0000115>
        <oboInOwl:hasOBONamespace>GAZ</oboInOwl:hasOBONamespace>
        <oboInOwl:id>GAZ:00193812</oboInOwl:id>
        <rdfs:label>Yotvata Hai-Bar Nature Reserve</rdfs:label>
    </owl:NamedIndividual>
    


    <!-- http://purl.obolibrary.org/obo/GAZ_00193813 -->

    <owl:NamedIndividual rdf:about="http://purl.obolibrary.org/obo/GAZ_00193813">
        <obo:RO_0001025 rdf:resource="http://purl.obolibrary.org/obo/GAZ_00002711"/>
        <obo:RO_0001025 rdf:resource="http://purl.obolibrary.org/obo/GAZ_00193814"/>
        <obo:IAO_0000115>A breeding and reacclimation center administered by the Israel Nature Reserves and National Parks Authority, situated in the Carmel mountains in Northwestern Israel.</obo:IAO_0000115>
        <oboInOwl:hasOBONamespace>GAZ</oboInOwl:hasOBONamespace>
        <oboInOwl:id>GAZ:00193813</oboInOwl:id>
        <rdfs:label>Carmel Hai-Bar Nature Reserve</rdfs:label>
    </owl:NamedIndividual>
    


    <!-- http://purl.obolibrary.org/obo/GAZ_00193814 -->

    <owl:NamedIndividual rdf:about="http://purl.obolibrary.org/obo/GAZ_00193814">
        <obo:RO_0001025 rdf:resource="http://purl.obolibrary.org/obo/GAZ_00002476"/>
        <obo:IAO_0000115>A coastal mountain range in northern Israel stretching from the Mediterranean Sea towards the southeast.</obo:IAO_0000115>
        <oboInOwl:hasOBONamespace>GAZ</oboInOwl:hasOBONamespace>
        <oboInOwl:id>GAZ:00193814</oboInOwl:id>
        <rdfs:label>Carmel Mountains</rdfs:label>
    </owl:NamedIndividual>
    


    <!-- http://purl.obolibrary.org/obo/GAZ_00193815 -->

    <owl:NamedIndividual rdf:about="http://purl.obolibrary.org/obo/GAZ_00193815">
        <obo:RO_0001025 rdf:resource="http://purl.obolibrary.org/obo/GAZ_00002710"/>
        <obo:RO_0001025 rdf:resource="http://purl.obolibrary.org/obo/GAZ_00078236"/>
        <obo:IAO_0000115>A psammosere ecosystem located close to the city of Ashdod on the Israeli Coastal Plain near the Mediterranean sea. It is located south of Tel Aviv.</obo:IAO_0000115>
        <oboInOwl:hasOBONamespace>GAZ</oboInOwl:hasOBONamespace>
        <oboInOwl:id>GAZ:00193815</oboInOwl:id>
        <rdfs:label>Ashdod Sand Dune</rdfs:label>
    </owl:NamedIndividual>
    


    <!-- http://purl.obolibrary.org/obo/GAZ_00193816 -->

    <owl:NamedIndividual rdf:about="http://purl.obolibrary.org/obo/GAZ_00193816">
        <obo:RO_0001025 rdf:resource="http://purl.obolibrary.org/obo/GAZ_00057703"/>
        <obo:IAO_0000115>A protected area.</obo:IAO_0000115>
        <oboInOwl:hasOBONamespace>GAZ</oboInOwl:hasOBONamespace>
        <oboInOwl:id>GAZ:00193816</oboInOwl:id>
        <rdfs:label>Ein Gedi National Park</rdfs:label>
    </owl:NamedIndividual>
    


    <!-- http://purl.obolibrary.org/obo/GAZ_00193817 -->

    <owl:NamedIndividual rdf:about="http://purl.obolibrary.org/obo/GAZ_00193817">
        <obo:RO_0001025 rdf:resource="http://purl.obolibrary.org/obo/GAZ_00193816"/>
        <obo:IAO_0000115>An oasis in Israel, located west of the Dead Sea, close to Masada and the caves of Qumran.</obo:IAO_0000115>
        <oboInOwl:hasOBONamespace>GAZ</oboInOwl:hasOBONamespace>
        <oboInOwl:id>GAZ:00193817</oboInOwl:id>
        <rdfs:label>Ein Gedi</rdfs:label>
    </owl:NamedIndividual>
    


    <!-- http://purl.obolibrary.org/obo/GAZ_00193818 -->

    <owl:NamedIndividual rdf:about="http://purl.obolibrary.org/obo/GAZ_00193818">
        <obo:RO_0001025 rdf:resource="http://purl.obolibrary.org/obo/GAZ_00193817"/>
        <obo:IAO_0000115>A river.</obo:IAO_0000115>
        <oboInOwl:hasOBONamespace>GAZ</oboInOwl:hasOBONamespace>
        <oboInOwl:id>GAZ:00193818</oboInOwl:id>
        <rdfs:label>Nachal David</rdfs:label>
    </owl:NamedIndividual>
    


    <!-- http://purl.obolibrary.org/obo/GAZ_00193819 -->

    <owl:NamedIndividual rdf:about="http://purl.obolibrary.org/obo/GAZ_00193819">
        <obo:RO_0001025 rdf:resource="http://purl.obolibrary.org/obo/GAZ_00193817"/>
        <obo:IAO_0000115>A spring.</obo:IAO_0000115>
        <oboInOwl:hasOBONamespace>GAZ</oboInOwl:hasOBONamespace>
        <oboInOwl:id>GAZ:00193819</oboInOwl:id>
        <rdfs:label>Ein Gedi Spring</rdfs:label>
    </owl:NamedIndividual>
    


    <!-- http://purl.obolibrary.org/obo/GAZ_00193820 -->

    <owl:NamedIndividual rdf:about="http://purl.obolibrary.org/obo/GAZ_00193820">
        <obo:RO_0001025 rdf:resource="http://purl.obolibrary.org/obo/GAZ_00193817"/>
        <obo:IAO_0000115>A river.</obo:IAO_0000115>
        <oboInOwl:hasOBONamespace>GAZ</oboInOwl:hasOBONamespace>
        <oboInOwl:id>GAZ:00193820</oboInOwl:id>
        <rdfs:label>Nachal Arugot</rdfs:label>
    </owl:NamedIndividual>
    


    <!-- http://purl.obolibrary.org/obo/GAZ_00193821 -->

    <owl:NamedIndividual rdf:about="http://purl.obolibrary.org/obo/GAZ_00193821">
        <obo:RO_0001025 rdf:resource="http://purl.obolibrary.org/obo/GAZ_00193817"/>
        <obo:IAO_0000115>A spring.</obo:IAO_0000115>
        <oboInOwl:hasOBONamespace>GAZ</oboInOwl:hasOBONamespace>
        <oboInOwl:id>GAZ:00193821</oboInOwl:id>
        <rdfs:label>Shulamit Spring</rdfs:label>
    </owl:NamedIndividual>
    


    <!-- http://purl.obolibrary.org/obo/GAZ_00193822 -->

    <owl:NamedIndividual rdf:about="http://purl.obolibrary.org/obo/GAZ_00193822">
        <obo:RO_0001025 rdf:resource="http://purl.obolibrary.org/obo/GAZ_00002714"/>
        <obo:IAO_0000115>A Biblical garden located near Modi&apos;in, mid-way between Jerusalem and Tel Aviv, Israel.</obo:IAO_0000115>
        <oboInOwl:hasOBONamespace>GAZ</oboInOwl:hasOBONamespace>
        <oboInOwl:id>GAZ:00193822</oboInOwl:id>
        <rdfs:label>Neot Kedumim</rdfs:label>
    </owl:NamedIndividual>
    


    <!-- http://purl.obolibrary.org/obo/GAZ_00193823 -->

    <owl:NamedIndividual rdf:about="http://purl.obolibrary.org/obo/GAZ_00193823">
        <obo:RO_0001025 rdf:resource="http://purl.obolibrary.org/obo/GAZ_00002711"/>
        <obo:IAO_0000115>A protected area. An archeological site. It borders the town of Kiryat Tiv&apos;on on the northeast and is located close to the modern moshav of Beit She&apos;arim.</obo:IAO_0000115>
        <oboInOwl:hasOBONamespace>GAZ</oboInOwl:hasOBONamespace>
        <oboInOwl:id>GAZ:00193823</oboInOwl:id>
        <rdfs:label>Beit She&apos;arim National Park</rdfs:label>
    </owl:NamedIndividual>
    


    <!-- http://purl.obolibrary.org/obo/GAZ_00193824 -->

    <owl:NamedIndividual rdf:about="http://purl.obolibrary.org/obo/GAZ_00193824">
        <obo:RO_0001025 rdf:resource="http://purl.obolibrary.org/obo/GAZ_00057704"/>
        <obo:IAO_0000115>The largest wadi of the Negev Desert.</obo:IAO_0000115>
        <oboInOwl:hasOBONamespace>GAZ</oboInOwl:hasOBONamespace>
        <oboInOwl:id>GAZ:00193824</oboInOwl:id>
        <rdfs:label>Nahal Zin</rdfs:label>
    </owl:NamedIndividual>
    


    <!-- http://purl.obolibrary.org/obo/GAZ_00193825 -->

    <owl:NamedIndividual rdf:about="http://purl.obolibrary.org/obo/GAZ_00193825">
        <obo:RO_0001025 rdf:resource="http://purl.obolibrary.org/obo/GAZ_00193824"/>
        <obo:IAO_0000115>A canyon in the Negev Desert of Israel, south of the kibbutz Sde Boker.</obo:IAO_0000115>
        <oboInOwl:hasOBONamespace>GAZ</oboInOwl:hasOBONamespace>
        <oboInOwl:id>GAZ:00193825</oboInOwl:id>
        <rdfs:label>Ein Avdat Canyon</rdfs:label>
    </owl:NamedIndividual>
    


    <!-- http://purl.obolibrary.org/obo/GAZ_00193826 -->

    <owl:NamedIndividual rdf:about="http://purl.obolibrary.org/obo/GAZ_00193826">
        <obo:RO_0001025 rdf:resource="http://purl.obolibrary.org/obo/GAZ_00193805"/>
        <obo:IAO_0000115>The southernmost spring in the Ein Avdat Canyon.</obo:IAO_0000115>
        <oboInOwl:hasOBONamespace>GAZ</oboInOwl:hasOBONamespace>
        <oboInOwl:id>GAZ:00193826</oboInOwl:id>
        <rdfs:label>Ein Ma&apos;arif</rdfs:label>
    </owl:NamedIndividual>
    


    <!-- http://purl.obolibrary.org/obo/GAZ_00193827 -->

    <owl:NamedIndividual rdf:about="http://purl.obolibrary.org/obo/GAZ_00193827">
        <obo:RO_0001025 rdf:resource="http://purl.obolibrary.org/obo/GAZ_00193805"/>
        <obo:IAO_0000115>A spring.</obo:IAO_0000115>
        <oboInOwl:hasOBONamespace>GAZ</oboInOwl:hasOBONamespace>
        <oboInOwl:id>GAZ:00193827</oboInOwl:id>
        <rdfs:label>Ein Mor</rdfs:label>
    </owl:NamedIndividual>
    


    <!-- http://purl.obolibrary.org/obo/GAZ_00193828 -->

    <owl:NamedIndividual rdf:about="http://purl.obolibrary.org/obo/GAZ_00193828">
        <obo:RO_0001025 rdf:resource="http://purl.obolibrary.org/obo/GAZ_00002713"/>
        <obo:IAO_0000115>A protected area. Located near Beit She&apos;an.</obo:IAO_0000115>
        <oboInOwl:hasOBONamespace>GAZ</oboInOwl:hasOBONamespace>
        <oboInOwl:id>GAZ:00193828</oboInOwl:id>
        <rdfs:label>Gan HaShlosha National Park</rdfs:label>
    </owl:NamedIndividual>
    


    <!-- http://purl.obolibrary.org/obo/GAZ_00193829 -->

    <owl:NamedIndividual rdf:about="http://purl.obolibrary.org/obo/GAZ_00193829">
        <obo:RO_0001025 rdf:resource="http://purl.obolibrary.org/obo/GAZ_00002712"/>
        <obo:RO_0001025 rdf:resource="http://purl.obolibrary.org/obo/GAZ_00057703"/>
        <obo:IAO_0000115>A protected area. Located on a dry plateau about a mile inland from the northwestern shore of the Dead Sea in the West Bank, just next to the Israeli kibbutz of Kalia. An archeological site.</obo:IAO_0000115>
        <oboInOwl:hasOBONamespace>GAZ</oboInOwl:hasOBONamespace>
        <oboInOwl:id>GAZ:00193829</oboInOwl:id>
        <rdfs:label>Qumran National Park</rdfs:label>
    </owl:NamedIndividual>
    


    <!-- http://purl.obolibrary.org/obo/GAZ_00193830 -->

    <owl:NamedIndividual rdf:about="http://purl.obolibrary.org/obo/GAZ_00193830">
        <obo:RO_0001025 rdf:resource="http://purl.obolibrary.org/obo/GAZ_00078270"/>
        <obo:IAO_0000115>An urban park located in Tel Aviv, Israel. Lying between Rokach Boulevard and the Bavli neighborhood.</obo:IAO_0000115>
        <oboInOwl:hasOBONamespace>GAZ</oboInOwl:hasOBONamespace>
        <oboInOwl:id>GAZ:00193830</oboInOwl:id>
        <rdfs:label>Yarkon Park</rdfs:label>
    </owl:NamedIndividual>
    


    <!-- http://purl.obolibrary.org/obo/GAZ_00193831 -->

    <owl:NamedIndividual rdf:about="http://purl.obolibrary.org/obo/GAZ_00193831">
        <obo:RO_0001025 rdf:resource="http://purl.obolibrary.org/obo/GAZ_00002712"/>
        <obo:RO_0001025 rdf:resource="http://purl.obolibrary.org/obo/GAZ_00057703"/>
        <obo:IAO_0000115>A protected area.</obo:IAO_0000115>
        <oboInOwl:hasOBONamespace>GAZ</oboInOwl:hasOBONamespace>
        <oboInOwl:id>GAZ:00193831</oboInOwl:id>
        <rdfs:label>En Prat (En Fara) Nature Reserve</rdfs:label>
    </owl:NamedIndividual>
    


    <!-- http://purl.obolibrary.org/obo/GAZ_00193832 -->

    <owl:NamedIndividual rdf:about="http://purl.obolibrary.org/obo/GAZ_00193832">
        <obo:RO_0001025 rdf:resource="http://purl.obolibrary.org/obo/GAZ_00193831"/>
        <obo:IAO_0000115>A spring.</obo:IAO_0000115>
        <oboInOwl:hasOBONamespace>GAZ</oboInOwl:hasOBONamespace>
        <oboInOwl:id>GAZ:00193832</oboInOwl:id>
        <rdfs:label>En Prat</rdfs:label>
    </owl:NamedIndividual>
    


    <!-- http://purl.obolibrary.org/obo/GAZ_00193833 -->

    <owl:NamedIndividual rdf:about="http://purl.obolibrary.org/obo/GAZ_00193833">
        <obo:RO_0001025 rdf:resource="http://purl.obolibrary.org/obo/GAZ_00002712"/>
        <obo:RO_0001025 rdf:resource="http://purl.obolibrary.org/obo/GAZ_00057703"/>
        <obo:IAO_0000115>A protected area. An archeological site. Located south of Jerusalem and east of Bethlehem, on the edge of the Judean Desert.</obo:IAO_0000115>
        <oboInOwl:hasOBONamespace>GAZ</oboInOwl:hasOBONamespace>
        <oboInOwl:id>GAZ:00193833</oboInOwl:id>
        <rdfs:label>Herodium (Herodion) National Park</rdfs:label>
    </owl:NamedIndividual>
    


    <!-- http://purl.obolibrary.org/obo/GAZ_00193834 -->

    <owl:NamedIndividual rdf:about="http://purl.obolibrary.org/obo/GAZ_00193834">
        <obo:RO_0001025 rdf:resource="http://purl.obolibrary.org/obo/GAZ_00002712"/>
        <obo:IAO_0000115>A protected area. An archeological site. Located some 12 km north of the city of Shechem, on the main road to Jenin near the Arab village of Sebastia.</obo:IAO_0000115>
        <oboInOwl:hasOBONamespace>GAZ</oboInOwl:hasOBONamespace>
        <oboInOwl:id>GAZ:00193834</oboInOwl:id>
        <rdfs:label>Shomron National Park (Sebastia)</rdfs:label>
    </owl:NamedIndividual>
    


    <!-- http://purl.obolibrary.org/obo/GAZ_00193835 -->

    <owl:NamedIndividual rdf:about="http://purl.obolibrary.org/obo/GAZ_00193835">
        <obo:RO_0001025 rdf:resource="http://purl.obolibrary.org/obo/GAZ_00057703"/>
        <obo:IAO_0000115>A protected area on the shores of the Dead Sea.</obo:IAO_0000115>
        <oboInOwl:hasOBONamespace>GAZ</oboInOwl:hasOBONamespace>
        <oboInOwl:id>GAZ:00193835</oboInOwl:id>
        <rdfs:label>Enot Tsukim Nature Reserve</rdfs:label>
    </owl:NamedIndividual>
    


    <!-- http://purl.obolibrary.org/obo/GAZ_00193836 -->

    <owl:NamedIndividual rdf:about="http://purl.obolibrary.org/obo/GAZ_00193836">
        <obo:RO_0001025 rdf:resource="http://purl.obolibrary.org/obo/GAZ_00057703"/>
        <obo:IAO_0000115>A protected area. An archeological site. A World Heritage Site.</obo:IAO_0000115>
        <oboInOwl:hasOBONamespace>GAZ</oboInOwl:hasOBONamespace>
        <oboInOwl:id>GAZ:00193836</oboInOwl:id>
        <rdfs:label>Masada National Park</rdfs:label>
    </owl:NamedIndividual>
    


    <!-- http://purl.obolibrary.org/obo/GAZ_00193837 -->

    <owl:NamedIndividual rdf:about="http://purl.obolibrary.org/obo/GAZ_00193837">
        <obo:RO_0001025 rdf:resource="http://purl.obolibrary.org/obo/GAZ_00193835"/>
        <obo:IAO_0000115>A part of Enot Tsukim Nature Reserve.</obo:IAO_0000115>
        <oboInOwl:hasOBONamespace>GAZ</oboInOwl:hasOBONamespace>
        <oboInOwl:id>GAZ:00193837</oboInOwl:id>
        <rdfs:label>Vistors Reserve, Enot Tsukim Nature Reserve</rdfs:label>
    </owl:NamedIndividual>
    


    <!-- http://purl.obolibrary.org/obo/GAZ_00193838 -->

    <owl:NamedIndividual rdf:about="http://purl.obolibrary.org/obo/GAZ_00193838">
        <obo:RO_0001025 rdf:resource="http://purl.obolibrary.org/obo/GAZ_00193835"/>
        <obo:IAO_0000115>A part of Enot Tsukim Nature Reserve.</obo:IAO_0000115>
        <oboInOwl:hasOBONamespace>GAZ</oboInOwl:hasOBONamespace>
        <oboInOwl:id>GAZ:00193838</oboInOwl:id>
        <rdfs:label>Souther Hidden Reserve, Enot Tsukim Nature Reserve</rdfs:label>
    </owl:NamedIndividual>
    


    <!-- http://purl.obolibrary.org/obo/GAZ_00193839 -->

    <owl:NamedIndividual rdf:about="http://purl.obolibrary.org/obo/GAZ_00193839">
        <obo:RO_0001025 rdf:resource="http://purl.obolibrary.org/obo/GAZ_00193835"/>
        <oboInOwl:hasOBONamespace>GAZ</oboInOwl:hasOBONamespace>
        <oboInOwl:id>GAZ:00193839</oboInOwl:id>
        <rdfs:label>Northern Closed Reserve, Enot Tsukim Nature Reserve</rdfs:label>
    </owl:NamedIndividual>
    


    <!-- http://purl.obolibrary.org/obo/GAZ_00193840 -->

    <owl:NamedIndividual rdf:about="http://purl.obolibrary.org/obo/GAZ_00193840">
        <obo:RO_0001025 rdf:resource="http://purl.obolibrary.org/obo/GAZ_00002714"/>
        <obo:IAO_0000115>A protected area. Located on the northern coastal plain north of Netanya.</obo:IAO_0000115>
        <oboInOwl:hasOBONamespace>GAZ</oboInOwl:hasOBONamespace>
        <oboInOwl:id>GAZ:00193840</oboInOwl:id>
        <rdfs:label>Alexander Stream Hof Bet Yanai National Park</rdfs:label>
    </owl:NamedIndividual>
    


    <!-- http://purl.obolibrary.org/obo/GAZ_00193841 -->

    <owl:NamedIndividual rdf:about="http://purl.obolibrary.org/obo/GAZ_00193841">
        <obo:RO_0001025 rdf:resource="http://purl.obolibrary.org/obo/GAZ_00193840"/>
        <obo:IAO_0000115>A river.</obo:IAO_0000115>
        <oboInOwl:hasOBONamespace>GAZ</oboInOwl:hasOBONamespace>
        <oboInOwl:id>GAZ:00193841</oboInOwl:id>
        <rdfs:label>Alexander Stream</rdfs:label>
    </owl:NamedIndividual>
    


    <!-- http://purl.obolibrary.org/obo/GAZ_00193842 -->

    <owl:NamedIndividual rdf:about="http://purl.obolibrary.org/obo/GAZ_00193842">
        <obo:RO_0001025 rdf:resource="http://purl.obolibrary.org/obo/GAZ_00078213"/>
        <obo:IAO_0000115>A protected area. An archeological site. Located north of Hertsliya Pituah on the coastal plain.</obo:IAO_0000115>
        <oboInOwl:hasOBONamespace>GAZ</oboInOwl:hasOBONamespace>
        <oboInOwl:id>GAZ:00193842</oboInOwl:id>
        <rdfs:label>Apollonia National Park</rdfs:label>
    </owl:NamedIndividual>
    


    <!-- http://purl.obolibrary.org/obo/GAZ_00193843 -->

    <owl:NamedIndividual rdf:about="http://purl.obolibrary.org/obo/GAZ_00193843">
        <obo:RO_0001025 rdf:resource="http://purl.obolibrary.org/obo/GAZ_00002476"/>
        <obo:IAO_0000115>A protected area.</obo:IAO_0000115>
        <oboInOwl:hasOBONamespace>GAZ</oboInOwl:hasOBONamespace>
        <oboInOwl:id>GAZ:00193843</oboInOwl:id>
        <rdfs:label>Bet Guvrin-Maresha National Park</rdfs:label>
    </owl:NamedIndividual>
    


    <!-- http://purl.obolibrary.org/obo/GAZ_00193844 -->

    <owl:NamedIndividual rdf:about="http://purl.obolibrary.org/obo/GAZ_00193844">
        <obo:RO_0001025 rdf:resource="http://purl.obolibrary.org/obo/GAZ_00002714"/>
        <obo:IAO_0000115>A protected area. An archeological site. Located on a hill known as Mount Ma&apos;oz overlooking the Tel Aviv-Jerusalem highway.</obo:IAO_0000115>
        <oboInOwl:hasOBONamespace>GAZ</oboInOwl:hasOBONamespace>
        <oboInOwl:id>GAZ:00193844</oboInOwl:id>
        <rdfs:label>Castel National Park</rdfs:label>
    </owl:NamedIndividual>
    


    <!-- http://purl.obolibrary.org/obo/GAZ_00193845 -->

    <owl:NamedIndividual rdf:about="http://purl.obolibrary.org/obo/GAZ_00193845">
        <obo:RO_0001025 rdf:resource="http://purl.obolibrary.org/obo/GAZ_00002476"/>
        <obo:IAO_0000115>A protected area. An archeological site.</obo:IAO_0000115>
        <oboInOwl:hasOBONamespace>GAZ</oboInOwl:hasOBONamespace>
        <oboInOwl:id>GAZ:00193845</oboInOwl:id>
        <rdfs:label>En Hemed (Aqua Bella) National Park</rdfs:label>
    </owl:NamedIndividual>
    


    <!-- http://purl.obolibrary.org/obo/GAZ_00193846 -->

    <owl:NamedIndividual rdf:about="http://purl.obolibrary.org/obo/GAZ_00193846">
        <obo:RO_0001025 rdf:resource="http://purl.obolibrary.org/obo/GAZ_00002476"/>
        <obo:IAO_0000115>A protected area.</obo:IAO_0000115>
        <oboInOwl:hasOBONamespace>GAZ</oboInOwl:hasOBONamespace>
        <oboInOwl:id>GAZ:00193846</oboInOwl:id>
        <rdfs:label>Stalactite Cave Nature Reserve</rdfs:label>
    </owl:NamedIndividual>
    


    <!-- http://purl.obolibrary.org/obo/GAZ_00193847 -->

    <owl:NamedIndividual rdf:about="http://purl.obolibrary.org/obo/GAZ_00193847">
        <obo:RO_0001025 rdf:resource="http://purl.obolibrary.org/obo/GAZ_00193846"/>
        <obo:IAO_0000115>A limestone cave.</obo:IAO_0000115>
        <oboInOwl:hasOBONamespace>GAZ</oboInOwl:hasOBONamespace>
        <oboInOwl:id>GAZ:00193847</oboInOwl:id>
        <rdfs:label>Stalactite Cave</rdfs:label>
    </owl:NamedIndividual>
    


    <!-- http://purl.obolibrary.org/obo/GAZ_00193848 -->

    <owl:NamedIndividual rdf:about="http://purl.obolibrary.org/obo/GAZ_00193848">
        <obo:RO_0001025 rdf:resource="http://purl.obolibrary.org/obo/GAZ_00002476"/>
        <obo:IAO_0000115>A protected area. An archeological site. Located east of Tel Aviv.</obo:IAO_0000115>
        <oboInOwl:hasOBONamespace>GAZ</oboInOwl:hasOBONamespace>
        <oboInOwl:id>GAZ:00193848</oboInOwl:id>
        <rdfs:label>Yarkon and Tel Afek National Park</rdfs:label>
    </owl:NamedIndividual>
    


    <!-- http://purl.obolibrary.org/obo/GAZ_00193849 -->

    <owl:NamedIndividual rdf:about="http://purl.obolibrary.org/obo/GAZ_00193849">
        <obo:RO_0001025 rdf:resource="http://purl.obolibrary.org/obo/GAZ_00002713"/>
        <obo:IAO_0000115>A protected area. An archeological site. Located in the hills of Lower Galilee, west of Nazareth.</obo:IAO_0000115>
        <oboInOwl:hasOBONamespace>GAZ</oboInOwl:hasOBONamespace>
        <oboInOwl:id>GAZ:00193849</oboInOwl:id>
        <rdfs:label>Zippori National Park</rdfs:label>
    </owl:NamedIndividual>
    


    <!-- http://purl.obolibrary.org/obo/GAZ_00193850 -->

    <owl:NamedIndividual rdf:about="http://purl.obolibrary.org/obo/GAZ_00193850">
        <obo:RO_0001025 rdf:resource="http://purl.obolibrary.org/obo/GAZ_00002713"/>
        <obo:IAO_0000115>A protected area. Located in the Bethsaida Valley, northeast of the Sea of Galilee.</obo:IAO_0000115>
        <oboInOwl:hasOBONamespace>GAZ</oboInOwl:hasOBONamespace>
        <oboInOwl:id>GAZ:00193850</oboInOwl:id>
        <rdfs:label>Betekha, Bethsaida, Majrase and Zaki Nature Reserve</rdfs:label>
    </owl:NamedIndividual>
    


    <!-- http://purl.obolibrary.org/obo/GAZ_00193851 -->

    <owl:NamedIndividual rdf:about="http://purl.obolibrary.org/obo/GAZ_00193851">
        <obo:RO_0001025 rdf:resource="http://purl.obolibrary.org/obo/GAZ_00002476"/>
        <obo:IAO_0000115>A protected area.</obo:IAO_0000115>
        <oboInOwl:hasOBONamespace>GAZ</oboInOwl:hasOBONamespace>
        <oboInOwl:id>GAZ:00193851</oboInOwl:id>
        <rdfs:label>Taninim Nature Reserve</rdfs:label>
    </owl:NamedIndividual>
    


    <!-- http://purl.obolibrary.org/obo/GAZ_00193852 -->

    <owl:NamedIndividual rdf:about="http://purl.obolibrary.org/obo/GAZ_00193852">
        <obo:RO_0001025 rdf:resource="http://purl.obolibrary.org/obo/GAZ_00193851"/>
        <obo:IAO_0000115>A river located in Israel, originating near Ramot Menashe and discharging to the Mediterranean Sea south of Ma&apos;agan Michael.</obo:IAO_0000115>
        <oboInOwl:hasOBONamespace>GAZ</oboInOwl:hasOBONamespace>
        <oboInOwl:id>GAZ:00193852</oboInOwl:id>
        <rdfs:label>Taninim Stream</rdfs:label>
    </owl:NamedIndividual>
    


    <!-- http://purl.obolibrary.org/obo/GAZ_00193853 -->

    <owl:NamedIndividual rdf:about="http://purl.obolibrary.org/obo/GAZ_00193853">
        <obo:RO_0001025 rdf:resource="http://purl.obolibrary.org/obo/GAZ_00193814"/>
        <obo:IAO_0000115>A protected area.</obo:IAO_0000115>
        <oboInOwl:hasOBONamespace>GAZ</oboInOwl:hasOBONamespace>
        <oboInOwl:id>GAZ:00193853</oboInOwl:id>
        <rdfs:label>Mount Carmel National Park</rdfs:label>
    </owl:NamedIndividual>
    


    <!-- http://purl.obolibrary.org/obo/GAZ_00193854 -->

    <owl:NamedIndividual rdf:about="http://purl.obolibrary.org/obo/GAZ_00193854">
        <obo:RO_0001025 rdf:resource="http://purl.obolibrary.org/obo/GAZ_00010533"/>
        <obo:IAO_0000115>A protected area. An archeological site. A World Heritage Site.</obo:IAO_0000115>
        <oboInOwl:hasOBONamespace>GAZ</oboInOwl:hasOBONamespace>
        <oboInOwl:id>GAZ:00193854</oboInOwl:id>
        <rdfs:label>Megiddo National Park</rdfs:label>
    </owl:NamedIndividual>
    


    <!-- http://purl.obolibrary.org/obo/GAZ_00193855 -->

    <owl:NamedIndividual rdf:about="http://purl.obolibrary.org/obo/GAZ_00193855">
        <obo:RO_0001025 rdf:resource="http://purl.obolibrary.org/obo/GAZ_00010533"/>
        <obo:IAO_0000115>A protected area. An archeological site.</obo:IAO_0000115>
        <oboInOwl:hasOBONamespace>GAZ</oboInOwl:hasOBONamespace>
        <oboInOwl:id>GAZ:00193855</oboInOwl:id>
        <rdfs:label>Ma&apos;ayan Harod National Park</rdfs:label>
    </owl:NamedIndividual>
    


    <!-- http://purl.obolibrary.org/obo/GAZ_00193856 -->

    <owl:NamedIndividual rdf:about="http://purl.obolibrary.org/obo/GAZ_00193856">
        <obo:RO_0001025 rdf:resource="http://purl.obolibrary.org/obo/GAZ_00193855"/>
        <obo:IAO_0000115>A spring. It emerges from a rocky cave on the slope of Mount Gilboa.</obo:IAO_0000115>
        <oboInOwl:hasOBONamespace>GAZ</oboInOwl:hasOBONamespace>
        <oboInOwl:id>GAZ:00193856</oboInOwl:id>
        <rdfs:label>Ma&apos;ayan Harod</rdfs:label>
    </owl:NamedIndividual>
    


    <!-- http://purl.obolibrary.org/obo/GAZ_00193857 -->

    <owl:NamedIndividual rdf:about="http://purl.obolibrary.org/obo/GAZ_00193857">
        <obo:RO_0001025 rdf:resource="http://purl.obolibrary.org/obo/GAZ_00002476"/>
        <obo:IAO_0000115>A protected area. An archeological site. Located E of the Sea of Galilee.</obo:IAO_0000115>
        <oboInOwl:hasOBONamespace>GAZ</oboInOwl:hasOBONamespace>
        <oboInOwl:id>GAZ:00193857</oboInOwl:id>
        <rdfs:label>Kursi National Park</rdfs:label>
    </owl:NamedIndividual>
    


    <!-- http://purl.obolibrary.org/obo/GAZ_00193858 -->

    <owl:NamedIndividual rdf:about="http://purl.obolibrary.org/obo/GAZ_00193858">
        <obo:RO_0001025 rdf:resource="http://purl.obolibrary.org/obo/GAZ_00002711"/>
        <obo:IAO_0000115>A protected area. Located in the Acre Valley near the Haifa Bay suburb of Kiryat Bialik. It is the last remnant of the Na&apos;aman Stream wetlands.</obo:IAO_0000115>
        <oboInOwl:hasOBONamespace>GAZ</oboInOwl:hasOBONamespace>
        <oboInOwl:id>GAZ:00193858</oboInOwl:id>
        <rdfs:label>En Afek Nature Reserve</rdfs:label>
    </owl:NamedIndividual>
    


    <!-- http://purl.obolibrary.org/obo/GAZ_00193859 -->

    <owl:NamedIndividual rdf:about="http://purl.obolibrary.org/obo/GAZ_00193859">
        <obo:RO_0001025 rdf:resource="http://purl.obolibrary.org/obo/GAZ_00002713"/>
        <obo:IAO_0000115>A protected area. An archeological site.</obo:IAO_0000115>
        <oboInOwl:hasOBONamespace>GAZ</oboInOwl:hasOBONamespace>
        <oboInOwl:id>GAZ:00193859</oboInOwl:id>
        <rdfs:label>Hamat Tiberias National Park</rdfs:label>
    </owl:NamedIndividual>
    


    <!-- http://purl.obolibrary.org/obo/GAZ_00193860 -->

    <owl:NamedIndividual rdf:about="http://purl.obolibrary.org/obo/GAZ_00193860">
        <obo:RO_0001025 rdf:resource="http://purl.obolibrary.org/obo/GAZ_00193814"/>
        <obo:IAO_0000115>A protected area.</obo:IAO_0000115>
        <oboInOwl:hasOBONamespace>GAZ</oboInOwl:hasOBONamespace>
        <oboInOwl:id>GAZ:00193860</oboInOwl:id>
        <rdfs:label>Hai Bar Carmel</rdfs:label>
    </owl:NamedIndividual>
    


    <!-- http://purl.obolibrary.org/obo/GAZ_00193861 -->

    <owl:NamedIndividual rdf:about="http://purl.obolibrary.org/obo/GAZ_00193861">
        <obo:RO_0001025 rdf:resource="http://purl.obolibrary.org/obo/GAZ_00002476"/>
        <obo:IAO_0000115>A protected area.</obo:IAO_0000115>
        <oboInOwl:hasOBONamespace>GAZ</oboInOwl:hasOBONamespace>
        <oboInOwl:id>GAZ:00193861</oboInOwl:id>
        <rdfs:label>Gan Hashlosha National Park (Sahne)</rdfs:label>
    </owl:NamedIndividual>
    


    <!-- http://purl.obolibrary.org/obo/GAZ_00193862 -->

    <owl:NamedIndividual rdf:about="http://purl.obolibrary.org/obo/GAZ_00193862">
        <obo:RO_0001025 rdf:resource="http://purl.obolibrary.org/obo/GAZ_00193858"/>
        <obo:IAO_0000115>A river.</obo:IAO_0000115>
        <oboInOwl:hasOBONamespace>GAZ</oboInOwl:hasOBONamespace>
        <oboInOwl:id>GAZ:00193862</oboInOwl:id>
        <rdfs:label>Na&apos;aman Stream</rdfs:label>
    </owl:NamedIndividual>
    


    <!-- http://purl.obolibrary.org/obo/GAZ_00193863 -->

    <owl:NamedIndividual rdf:about="http://purl.obolibrary.org/obo/GAZ_00193863">
        <obo:RO_0001025 rdf:resource="http://purl.obolibrary.org/obo/GAZ_00002476"/>
        <obo:IAO_0000115>A protected area. An archeological site.</obo:IAO_0000115>
        <oboInOwl:hasOBONamespace>GAZ</oboInOwl:hasOBONamespace>
        <oboInOwl:id>GAZ:00193863</oboInOwl:id>
        <rdfs:label>Capernaum National Park</rdfs:label>
    </owl:NamedIndividual>
    


    <!-- http://purl.obolibrary.org/obo/GAZ_00193864 -->

    <owl:NamedIndividual rdf:about="http://purl.obolibrary.org/obo/GAZ_00193864">
        <obo:RO_0001025 rdf:resource="http://purl.obolibrary.org/obo/GAZ_00002711"/>
        <obo:IAO_0000115>A protected area. An archeological site.</obo:IAO_0000115>
        <oboInOwl:hasOBONamespace>GAZ</oboInOwl:hasOBONamespace>
        <oboInOwl:id>GAZ:00193864</oboInOwl:id>
        <rdfs:label>Caesarea National Park</rdfs:label>
    </owl:NamedIndividual>
    


    <!-- http://purl.obolibrary.org/obo/GAZ_00193865 -->

    <owl:NamedIndividual rdf:about="http://purl.obolibrary.org/obo/GAZ_00193865">
        <obo:RO_0001025 rdf:resource="http://purl.obolibrary.org/obo/GAZ_00002476"/>
        <obo:IAO_0000115>A protected area. An archeological site.</obo:IAO_0000115>
        <oboInOwl:hasOBONamespace>GAZ</oboInOwl:hasOBONamespace>
        <oboInOwl:id>GAZ:00193865</oboInOwl:id>
        <rdfs:label>Bet She&apos;arim National Park</rdfs:label>
    </owl:NamedIndividual>
    


    <!-- http://purl.obolibrary.org/obo/GAZ_00193866 -->

    <owl:NamedIndividual rdf:about="http://purl.obolibrary.org/obo/GAZ_00193866">
        <obo:RO_0001025 rdf:resource="http://purl.obolibrary.org/obo/GAZ_00044915"/>
        <obo:IAO_0000115>A protected area. An archeological site.</obo:IAO_0000115>
        <oboInOwl:hasOBONamespace>GAZ</oboInOwl:hasOBONamespace>
        <oboInOwl:id>GAZ:00193866</oboInOwl:id>
        <rdfs:label>Bet She&apos;an National Park</rdfs:label>
    </owl:NamedIndividual>
    


    <!-- http://purl.obolibrary.org/obo/GAZ_00193867 -->

    <owl:NamedIndividual rdf:about="http://purl.obolibrary.org/obo/GAZ_00193867">
        <obo:RO_0001025 rdf:resource="http://purl.obolibrary.org/obo/GAZ_00002476"/>
        <obo:IAO_0000115>A protected area. An archeological site.</obo:IAO_0000115>
        <oboInOwl:hasOBONamespace>GAZ</oboInOwl:hasOBONamespace>
        <oboInOwl:id>GAZ:00193867</oboInOwl:id>
        <rdfs:label>Belvoir (Kokhav HaYarden) National Park</rdfs:label>
    </owl:NamedIndividual>
    


    <!-- http://purl.obolibrary.org/obo/GAZ_00193868 -->

    <owl:NamedIndividual rdf:about="http://purl.obolibrary.org/obo/GAZ_00193868">
        <obo:IAO_0000115>A protected area located in the central Golan Heights.</obo:IAO_0000115>
        <oboInOwl:hasOBONamespace>GAZ</oboInOwl:hasOBONamespace>
        <oboInOwl:id>GAZ:00193868</oboInOwl:id>
        <rdfs:label>Yehudiya Forest Nature Reserve</rdfs:label>
    </owl:NamedIndividual>
    


    <!-- http://purl.obolibrary.org/obo/GAZ_00193869 -->

    <owl:NamedIndividual rdf:about="http://purl.obolibrary.org/obo/GAZ_00193869">
        <obo:RO_0001025 rdf:resource="http://purl.obolibrary.org/obo/GAZ_00193868"/>
        <obo:IAO_0000115>A river.</obo:IAO_0000115>
        <oboInOwl:hasOBONamespace>GAZ</oboInOwl:hasOBONamespace>
        <oboInOwl:id>GAZ:00193869</oboInOwl:id>
        <rdfs:label>Meshushim Stream</rdfs:label>
    </owl:NamedIndividual>
    


    <!-- http://purl.obolibrary.org/obo/GAZ_00193870 -->

    <owl:NamedIndividual rdf:about="http://purl.obolibrary.org/obo/GAZ_00193870">
        <obo:RO_0001025 rdf:resource="http://purl.obolibrary.org/obo/GAZ_00193868"/>
        <obo:IAO_0000115>A river.</obo:IAO_0000115>
        <oboInOwl:hasOBONamespace>GAZ</oboInOwl:hasOBONamespace>
        <oboInOwl:id>GAZ:00193870</oboInOwl:id>
        <rdfs:label>Yehudiya Stream</rdfs:label>
    </owl:NamedIndividual>
    


    <!-- http://purl.obolibrary.org/obo/GAZ_00193871 -->

    <owl:NamedIndividual rdf:about="http://purl.obolibrary.org/obo/GAZ_00193871">
        <obo:RO_0001025 rdf:resource="http://purl.obolibrary.org/obo/GAZ_00193868"/>
        <obo:IAO_0000115>A river.</obo:IAO_0000115>
        <oboInOwl:hasOBONamespace>GAZ</oboInOwl:hasOBONamespace>
        <oboInOwl:id>GAZ:00193871</oboInOwl:id>
        <rdfs:label>Gamla Stream</rdfs:label>
    </owl:NamedIndividual>
    


    <!-- http://purl.obolibrary.org/obo/GAZ_00193872 -->

    <owl:NamedIndividual rdf:about="http://purl.obolibrary.org/obo/GAZ_00193872">
        <obo:RO_0001025 rdf:resource="http://purl.obolibrary.org/obo/GAZ_00193868"/>
        <obo:IAO_0000115>A river.</obo:IAO_0000115>
        <oboInOwl:hasOBONamespace>GAZ</oboInOwl:hasOBONamespace>
        <oboInOwl:id>GAZ:00193872</oboInOwl:id>
        <rdfs:label>Zavitan Stream</rdfs:label>
    </owl:NamedIndividual>
    


    <!-- http://purl.obolibrary.org/obo/GAZ_00193873 -->

    <owl:NamedIndividual rdf:about="http://purl.obolibrary.org/obo/GAZ_00193873">
        <obo:RO_0001025 rdf:resource="http://purl.obolibrary.org/obo/GAZ_00193868"/>
        <obo:IAO_0000115>A river.</obo:IAO_0000115>
        <oboInOwl:hasOBONamespace>GAZ</oboInOwl:hasOBONamespace>
        <oboInOwl:id>GAZ:00193873</oboInOwl:id>
        <rdfs:label>Daliyot Stream</rdfs:label>
    </owl:NamedIndividual>
    


    <!-- http://purl.obolibrary.org/obo/GAZ_00193874 -->

    <owl:NamedIndividual rdf:about="http://purl.obolibrary.org/obo/GAZ_00193874">
        <obo:RO_0001025 rdf:resource="http://purl.obolibrary.org/obo/GAZ_00078351"/>
        <obo:IAO_0000115>A Kibbutz located in the western Upper Galilee region of Israel, about 10 miles due east of the coastal town of Nahariya and five miles south of the border with Lebanon.</obo:IAO_0000115>
        <oboInOwl:hasOBONamespace>GAZ</oboInOwl:hasOBONamespace>
        <oboInOwl:id>GAZ:00193874</oboInOwl:id>
        <rdfs:label>Yehiam</rdfs:label>
    </owl:NamedIndividual>
    


    <!-- http://purl.obolibrary.org/obo/GAZ_00193875 -->

    <owl:NamedIndividual rdf:about="http://purl.obolibrary.org/obo/GAZ_00193875">
        <obo:RO_0001025 rdf:resource="http://purl.obolibrary.org/obo/GAZ_00193874"/>
        <obo:IAO_0000115>A protected area. An archeological site.</obo:IAO_0000115>
        <oboInOwl:hasOBONamespace>GAZ</oboInOwl:hasOBONamespace>
        <oboInOwl:id>GAZ:00193875</oboInOwl:id>
        <rdfs:label>Yehi&apos;am Fortress National Park</rdfs:label>
    </owl:NamedIndividual>
    


    <!-- http://purl.obolibrary.org/obo/GAZ_00193876 -->

    <owl:NamedIndividual rdf:about="http://purl.obolibrary.org/obo/GAZ_00193876">
        <obo:RO_0001025 rdf:resource="http://purl.obolibrary.org/obo/GAZ_00193868"/>
        <obo:IAO_0000115>A protected area.</obo:IAO_0000115>
        <oboInOwl:hasOBONamespace>GAZ</oboInOwl:hasOBONamespace>
        <oboInOwl:id>GAZ:00193876</oboInOwl:id>
        <rdfs:label>Meshushim Reserve</rdfs:label>
    </owl:NamedIndividual>
    


    <!-- http://purl.obolibrary.org/obo/GAZ_00193877 -->

    <owl:NamedIndividual rdf:about="http://purl.obolibrary.org/obo/GAZ_00193877">
        <obo:RO_0001025 rdf:resource="http://purl.obolibrary.org/obo/GAZ_00193876"/>
        <obo:IAO_0000115>A lake.</obo:IAO_0000115>
        <oboInOwl:hasOBONamespace>GAZ</oboInOwl:hasOBONamespace>
        <oboInOwl:id>GAZ:00193877</oboInOwl:id>
        <rdfs:label>Meshushim Pool</rdfs:label>
    </owl:NamedIndividual>
    


    <!-- http://purl.obolibrary.org/obo/GAZ_00193878 -->

    <owl:NamedIndividual rdf:about="http://purl.obolibrary.org/obo/GAZ_00193878">
        <obo:RO_0001025 rdf:resource="http://purl.obolibrary.org/obo/GAZ_00002713"/>
        <obo:IAO_0000115>A protected area.</obo:IAO_0000115>
        <oboInOwl:hasOBONamespace>GAZ</oboInOwl:hasOBONamespace>
        <oboInOwl:id>GAZ:00193878</oboInOwl:id>
        <rdfs:label>Iyon (Tanur) Stream Nature Reserve</rdfs:label>
    </owl:NamedIndividual>
    


    <!-- http://purl.obolibrary.org/obo/GAZ_00193879 -->

    <owl:NamedIndividual rdf:about="http://purl.obolibrary.org/obo/GAZ_00193879">
        <obo:RO_0001025 rdf:resource="http://purl.obolibrary.org/obo/GAZ_00008823"/>
        <obo:IAO_0000115>A protected area. An archeological site. Located opposite Kibbutz Ayelet HaShahar, between Rosh Pina and Metula.</obo:IAO_0000115>
        <oboInOwl:hasOBONamespace>GAZ</oboInOwl:hasOBONamespace>
        <oboInOwl:id>GAZ:00193879</oboInOwl:id>
        <rdfs:label>Tel Hazor National Park</rdfs:label>
    </owl:NamedIndividual>
    


    <!-- http://purl.obolibrary.org/obo/GAZ_00193880 -->

    <owl:NamedIndividual rdf:about="http://purl.obolibrary.org/obo/GAZ_00193880">
        <obo:RO_0001025 rdf:resource="http://purl.obolibrary.org/obo/GAZ_00002476"/>
        <obo:IAO_0000115>A protected area.</obo:IAO_0000115>
        <oboInOwl:hasOBONamespace>GAZ</oboInOwl:hasOBONamespace>
        <oboInOwl:id>GAZ:00193880</oboInOwl:id>
        <rdfs:label>Tel Dan Nature Reserve</rdfs:label>
    </owl:NamedIndividual>
    


    <!-- http://purl.obolibrary.org/obo/GAZ_00193881 -->

    <owl:NamedIndividual rdf:about="http://purl.obolibrary.org/obo/GAZ_00193881">
        <obo:RO_0001025 rdf:resource="http://purl.obolibrary.org/obo/GAZ_00002713"/>
        <obo:IAO_0000115>A protected area.</obo:IAO_0000115>
        <oboInOwl:hasOBONamespace>GAZ</oboInOwl:hasOBONamespace>
        <oboInOwl:id>GAZ:00193881</oboInOwl:id>
        <rdfs:label>Senir (Hatsbani) Stream Nature Reserve</rdfs:label>
    </owl:NamedIndividual>
    


    <!-- http://purl.obolibrary.org/obo/GAZ_00193882 -->

    <owl:NamedIndividual rdf:about="http://purl.obolibrary.org/obo/GAZ_00193882">
        <obo:IAO_0000115>A mountain in the Anti-Lebanon mountain range. The summit is on the border between Syria and Lebanon, and is under Syrian control. Part of the southern slopes of Mount Hermon fall within the Golan Heights.</obo:IAO_0000115>
        <oboInOwl:hasOBONamespace>GAZ</oboInOwl:hasOBONamespace>
        <oboInOwl:id>GAZ:00193882</oboInOwl:id>
        <rdfs:label>Mount Hermon</rdfs:label>
    </owl:NamedIndividual>
    


    <!-- http://purl.obolibrary.org/obo/GAZ_00193883 -->

    <owl:NamedIndividual rdf:about="http://purl.obolibrary.org/obo/GAZ_00193883">
        <obo:RO_0001025 rdf:resource="http://purl.obolibrary.org/obo/GAZ_00193882"/>
        <obo:IAO_0000115>An Israeili protected area. An archeological site. Located on the slopes of Mount Hermon above the Banias Spring.</obo:IAO_0000115>
        <oboInOwl:hasOBONamespace>GAZ</oboInOwl:hasOBONamespace>
        <oboInOwl:id>GAZ:00193883</oboInOwl:id>
        <rdfs:label>Nimrod Fortress National Park</rdfs:label>
    </owl:NamedIndividual>
    


    <!-- http://purl.obolibrary.org/obo/GAZ_00193884 -->

    <owl:NamedIndividual rdf:about="http://purl.obolibrary.org/obo/GAZ_00193884">
        <obo:RO_0001025 rdf:resource="http://purl.obolibrary.org/obo/GAZ_00002713"/>
        <obo:IAO_0000115>A protected area. An archeological site.</obo:IAO_0000115>
        <oboInOwl:hasOBONamespace>GAZ</oboInOwl:hasOBONamespace>
        <oboInOwl:id>GAZ:00193884</oboInOwl:id>
        <rdfs:label>Korazim National Park</rdfs:label>
    </owl:NamedIndividual>
    


    <!-- http://purl.obolibrary.org/obo/GAZ_00193885 -->

    <owl:NamedIndividual rdf:about="http://purl.obolibrary.org/obo/GAZ_00193885">
        <obo:RO_0001025 rdf:resource="http://purl.obolibrary.org/obo/GAZ_00008742"/>
        <obo:IAO_0000115>A protected area.</obo:IAO_0000115>
        <oboInOwl:hasOBONamespace>GAZ</oboInOwl:hasOBONamespace>
        <oboInOwl:id>GAZ:00193885</oboInOwl:id>
        <rdfs:label>Hurshat Tal National Park</rdfs:label>
    </owl:NamedIndividual>
    


    <!-- http://purl.obolibrary.org/obo/GAZ_00193886 -->

    <owl:NamedIndividual rdf:about="http://purl.obolibrary.org/obo/GAZ_00193886">
        <obo:RO_0001025 rdf:resource="http://purl.obolibrary.org/obo/GAZ_00008742"/>
        <obo:IAO_0000115>A protected area.</obo:IAO_0000115>
        <oboInOwl:hasOBONamespace>GAZ</oboInOwl:hasOBONamespace>
        <oboInOwl:id>GAZ:00193886</oboInOwl:id>
        <rdfs:label>Hula Nature Reserve</rdfs:label>
    </owl:NamedIndividual>
    


    <!-- http://purl.obolibrary.org/obo/GAZ_00193888 -->

    <owl:NamedIndividual rdf:about="http://purl.obolibrary.org/obo/GAZ_00193888">
        <obo:RO_0001025 rdf:resource="http://purl.obolibrary.org/obo/GAZ_00008823"/>
        <obo:IAO_0000115>A protected area.</obo:IAO_0000115>
        <oboInOwl:hasOBONamespace>GAZ</oboInOwl:hasOBONamespace>
        <oboInOwl:id>GAZ:00193888</oboInOwl:id>
        <rdfs:label>Hermon Stream (Banias) Nature Reserve</rdfs:label>
    </owl:NamedIndividual>
    


    <!-- http://purl.obolibrary.org/obo/GAZ_00193889 -->

    <owl:NamedIndividual rdf:about="http://purl.obolibrary.org/obo/GAZ_00193889">
        <obo:RO_0001025 rdf:resource="http://purl.obolibrary.org/obo/GAZ_00193888"/>
        <obo:IAO_0000115>A cave.</obo:IAO_0000115>
        <oboInOwl:hasOBONamespace>GAZ</oboInOwl:hasOBONamespace>
        <oboInOwl:id>GAZ:00193889</oboInOwl:id>
        <rdfs:label>Banias Cave</rdfs:label>
    </owl:NamedIndividual>
    


    <!-- http://purl.obolibrary.org/obo/GAZ_00193890 -->

    <owl:NamedIndividual rdf:about="http://purl.obolibrary.org/obo/GAZ_00193890">
        <obo:RO_0001025 rdf:resource="http://purl.obolibrary.org/obo/GAZ_00193888"/>
        <obo:IAO_0000115>A spring at the foot of Mount Hermon.</obo:IAO_0000115>
        <oboInOwl:hasOBONamespace>GAZ</oboInOwl:hasOBONamespace>
        <oboInOwl:id>GAZ:00193890</oboInOwl:id>
        <rdfs:label>Banias Spring</rdfs:label>
    </owl:NamedIndividual>
    


    <!-- http://purl.obolibrary.org/obo/GAZ_00193891 -->

    <owl:NamedIndividual rdf:about="http://purl.obolibrary.org/obo/GAZ_00193891">
        <obo:IAO_0000115>A protected area located in the central Golan Heights.</obo:IAO_0000115>
        <oboInOwl:hasOBONamespace>GAZ</oboInOwl:hasOBONamespace>
        <oboInOwl:id>GAZ:00193891</oboInOwl:id>
        <rdfs:label>Gamla Nature Reserve</rdfs:label>
    </owl:NamedIndividual>
    


    <!-- http://purl.obolibrary.org/obo/GAZ_00193892 -->

    <owl:NamedIndividual rdf:about="http://purl.obolibrary.org/obo/GAZ_00193892">
        <obo:RO_0001025 rdf:resource="http://purl.obolibrary.org/obo/GAZ_00002713"/>
        <obo:IAO_0000115>A protected area.</obo:IAO_0000115>
        <oboInOwl:hasOBONamespace>GAZ</oboInOwl:hasOBONamespace>
        <oboInOwl:id>GAZ:00193892</oboInOwl:id>
        <rdfs:label>Arbel National Park and Nature Reserve</rdfs:label>
    </owl:NamedIndividual>
    


    <!-- http://purl.obolibrary.org/obo/GAZ_00193893 -->

    <owl:NamedIndividual rdf:about="http://purl.obolibrary.org/obo/GAZ_00193893">
        <obo:RO_0001025 rdf:resource="http://purl.obolibrary.org/obo/GAZ_00002713"/>
        <obo:IAO_0000115>A protected area.</obo:IAO_0000115>
        <oboInOwl:hasOBONamespace>GAZ</oboInOwl:hasOBONamespace>
        <oboInOwl:id>GAZ:00193893</oboInOwl:id>
        <rdfs:label>Mount Meron Nature Reserve</rdfs:label>
    </owl:NamedIndividual>
    


    <!-- http://purl.obolibrary.org/obo/GAZ_00193894 -->

    <owl:NamedIndividual rdf:about="http://purl.obolibrary.org/obo/GAZ_00193894">
        <obo:RO_0001025 rdf:resource="http://purl.obolibrary.org/obo/GAZ_00193893"/>
        <obo:IAO_0000115>A protected area.</obo:IAO_0000115>
        <oboInOwl:hasOBONamespace>GAZ</oboInOwl:hasOBONamespace>
        <oboInOwl:id>GAZ:00193894</oboInOwl:id>
        <rdfs:label>Amud Stream Nature Reserve</rdfs:label>
    </owl:NamedIndividual>
    


    <!-- http://purl.obolibrary.org/obo/GAZ_00193895 -->

    <owl:NamedIndividual rdf:about="http://purl.obolibrary.org/obo/GAZ_00193895">
        <obo:RO_0001025 rdf:resource="http://purl.obolibrary.org/obo/GAZ_00193894"/>
        <obo:IAO_0000115>A spring.</obo:IAO_0000115>
        <oboInOwl:hasOBONamespace>GAZ</oboInOwl:hasOBONamespace>
        <oboInOwl:id>GAZ:00193895</oboInOwl:id>
        <rdfs:label>En Yakim</rdfs:label>
    </owl:NamedIndividual>
    


    <!-- http://purl.obolibrary.org/obo/GAZ_00193896 -->

    <owl:NamedIndividual rdf:about="http://purl.obolibrary.org/obo/GAZ_00193896">
        <obo:RO_0001025 rdf:resource="http://purl.obolibrary.org/obo/GAZ_00193894"/>
        <obo:IAO_0000115>A river.</obo:IAO_0000115>
        <oboInOwl:hasOBONamespace>GAZ</oboInOwl:hasOBONamespace>
        <oboInOwl:id>GAZ:00193896</oboInOwl:id>
        <rdfs:label>Amud Stream</rdfs:label>
    </owl:NamedIndividual>
    


    <!-- http://purl.obolibrary.org/obo/GAZ_00193897 -->

    <owl:NamedIndividual rdf:about="http://purl.obolibrary.org/obo/GAZ_00193897">
        <obo:RO_0001025 rdf:resource="http://purl.obolibrary.org/obo/GAZ_00002710"/>
        <obo:IAO_0000115>A forest at Shachariya, between Kiryat Gat and Lakhish Junction.</obo:IAO_0000115>
        <oboInOwl:hasOBONamespace>GAZ</oboInOwl:hasOBONamespace>
        <oboInOwl:id>GAZ:00193897</oboInOwl:id>
        <rdfs:label>Melachim Forest</rdfs:label>
    </owl:NamedIndividual>
    


    <!-- http://purl.obolibrary.org/obo/GAZ_00193898 -->

    <owl:NamedIndividual rdf:about="http://purl.obolibrary.org/obo/GAZ_00193898">
        <obo:RO_0001025 rdf:resource="http://purl.obolibrary.org/obo/GAZ_00002710"/>
        <obo:IAO_0000115>A forest near Amatzia.</obo:IAO_0000115>
        <oboInOwl:hasOBONamespace>GAZ</oboInOwl:hasOBONamespace>
        <oboInOwl:id>GAZ:00193898</oboInOwl:id>
        <rdfs:label>Amatzia Woodlands</rdfs:label>
    </owl:NamedIndividual>
    


    <!-- http://purl.obolibrary.org/obo/GAZ_00193899 -->

    <owl:NamedIndividual rdf:about="http://purl.obolibrary.org/obo/GAZ_00193899">
        <obo:RO_0001025 rdf:resource="http://purl.obolibrary.org/obo/GAZ_00057704"/>
        <obo:IAO_0000115>A forest in the N Negev.</obo:IAO_0000115>
        <oboInOwl:hasOBONamespace>GAZ</oboInOwl:hasOBONamespace>
        <oboInOwl:id>GAZ:00193899</oboInOwl:id>
        <rdfs:label>Lahav Forest</rdfs:label>
    </owl:NamedIndividual>
    


    <!-- http://purl.obolibrary.org/obo/GAZ_00193900 -->

    <owl:NamedIndividual rdf:about="http://purl.obolibrary.org/obo/GAZ_00193900">
        <obo:RO_0001025 rdf:resource="http://purl.obolibrary.org/obo/GAZ_00057704"/>
        <obo:IAO_0000115>A forest in the Negev. Located on Road No. 232 near Be&apos;eri from Hodiya Junction (Road No. 232) off Zikim-Karmia Road.</obo:IAO_0000115>
        <oboInOwl:hasOBONamespace>GAZ</oboInOwl:hasOBONamespace>
        <oboInOwl:id>GAZ:00193900</oboInOwl:id>
        <rdfs:label>Be&apos;eri Forest</rdfs:label>
    </owl:NamedIndividual>
    


    <!-- http://purl.obolibrary.org/obo/GAZ_00193901 -->

    <owl:NamedIndividual rdf:about="http://purl.obolibrary.org/obo/GAZ_00193901">
        <obo:RO_0001025 rdf:resource="http://purl.obolibrary.org/obo/GAZ_00057704"/>
        <obo:IAO_0000115>A forest in Israel, located on the southern slopes of Mount Hebron, on the edge of the Negev Desert.</obo:IAO_0000115>
        <oboInOwl:hasOBONamespace>GAZ</oboInOwl:hasOBONamespace>
        <oboInOwl:id>GAZ:00193901</oboInOwl:id>
        <rdfs:label>Yatir Forest</rdfs:label>
    </owl:NamedIndividual>
    


    <!-- http://purl.obolibrary.org/obo/GAZ_00193902 -->

    <owl:NamedIndividual rdf:about="http://purl.obolibrary.org/obo/GAZ_00193902">
        <obo:RO_0001025 rdf:resource="http://purl.obolibrary.org/obo/GAZ_00010532"/>
        <obo:IAO_0000115>A forest.</obo:IAO_0000115>
        <oboInOwl:hasOBONamespace>GAZ</oboInOwl:hasOBONamespace>
        <oboInOwl:id>GAZ:00193902</oboInOwl:id>
        <rdfs:label>Swiss Forest</rdfs:label>
    </owl:NamedIndividual>
    


    <!-- http://purl.obolibrary.org/obo/GAZ_00193903 -->

    <owl:NamedIndividual rdf:about="http://purl.obolibrary.org/obo/GAZ_00193903">
        <obo:RO_0001025 rdf:resource="http://purl.obolibrary.org/obo/GAZ_00010532"/>
        <obo:IAO_0000115>A forest.</obo:IAO_0000115>
        <oboInOwl:hasOBONamespace>GAZ</oboInOwl:hasOBONamespace>
        <oboInOwl:id>GAZ:00193903</oboInOwl:id>
        <rdfs:label>Tiberias Forest</rdfs:label>
    </owl:NamedIndividual>
    


    <!-- http://purl.obolibrary.org/obo/GAZ_00193904 -->

    <owl:NamedIndividual rdf:about="http://purl.obolibrary.org/obo/GAZ_00193904">
        <obo:RO_0001025 rdf:resource="http://purl.obolibrary.org/obo/GAZ_00008823"/>
        <obo:IAO_0000115>A forest.</obo:IAO_0000115>
        <oboInOwl:hasOBONamespace>GAZ</oboInOwl:hasOBONamespace>
        <oboInOwl:id>GAZ:00193904</oboInOwl:id>
        <rdfs:label>Mount Turan Forest</rdfs:label>
    </owl:NamedIndividual>
    


    <!-- http://purl.obolibrary.org/obo/GAZ_00193905 -->

    <owl:NamedIndividual rdf:about="http://purl.obolibrary.org/obo/GAZ_00193905">
        <obo:RO_0001025 rdf:resource="http://purl.obolibrary.org/obo/GAZ_00008823"/>
        <obo:IAO_0000115>A forest.</obo:IAO_0000115>
        <oboInOwl:hasOBONamespace>GAZ</oboInOwl:hasOBONamespace>
        <oboInOwl:id>GAZ:00193905</oboInOwl:id>
        <rdfs:label>Baram Forest</rdfs:label>
    </owl:NamedIndividual>
    


    <!-- http://purl.obolibrary.org/obo/GAZ_00193906 -->

    <owl:NamedIndividual rdf:about="http://purl.obolibrary.org/obo/GAZ_00193906">
        <obo:RO_0001025 rdf:resource="http://purl.obolibrary.org/obo/GAZ_00008823"/>
        <obo:IAO_0000115>A forest.</obo:IAO_0000115>
        <oboInOwl:hasOBONamespace>GAZ</oboInOwl:hasOBONamespace>
        <oboInOwl:id>GAZ:00193906</oboInOwl:id>
        <rdfs:label>Lavi Forest</rdfs:label>
    </owl:NamedIndividual>
    


    <!-- http://purl.obolibrary.org/obo/GAZ_00193907 -->

    <owl:NamedIndividual rdf:about="http://purl.obolibrary.org/obo/GAZ_00193907">
        <obo:RO_0001025 rdf:resource="http://purl.obolibrary.org/obo/GAZ_00002713"/>
        <obo:IAO_0000115>A forest in the Galilee region.</obo:IAO_0000115>
        <oboInOwl:hasOBONamespace>GAZ</oboInOwl:hasOBONamespace>
        <oboInOwl:id>GAZ:00193907</oboInOwl:id>
        <rdfs:label>Lower Hanita Forest</rdfs:label>
    </owl:NamedIndividual>
    


    <!-- http://purl.obolibrary.org/obo/GAZ_00193908 -->

    <owl:NamedIndividual rdf:about="http://purl.obolibrary.org/obo/GAZ_00193908">
        <obo:RO_0001025 rdf:resource="http://purl.obolibrary.org/obo/GAZ_00002713"/>
        <obo:IAO_0000115>A forest in the Galilee region.</obo:IAO_0000115>
        <oboInOwl:hasOBONamespace>GAZ</oboInOwl:hasOBONamespace>
        <oboInOwl:id>GAZ:00193908</oboInOwl:id>
        <rdfs:label>Biriya Forest</rdfs:label>
    </owl:NamedIndividual>
    


    <!-- http://purl.obolibrary.org/obo/GAZ_00193909 -->

    <owl:NamedIndividual rdf:about="http://purl.obolibrary.org/obo/GAZ_00193909">
        <obo:RO_0001025 rdf:resource="http://purl.obolibrary.org/obo/GAZ_00002713"/>
        <obo:IAO_0000115>A forest.</obo:IAO_0000115>
        <oboInOwl:hasOBONamespace>GAZ</oboInOwl:hasOBONamespace>
        <oboInOwl:id>GAZ:00193909</oboInOwl:id>
        <rdfs:label>Carmel Coast Forest</rdfs:label>
    </owl:NamedIndividual>
    


    <!-- http://purl.obolibrary.org/obo/GAZ_00193910 -->

    <owl:NamedIndividual rdf:about="http://purl.obolibrary.org/obo/GAZ_00193910">
        <obo:RO_0001025 rdf:resource="http://purl.obolibrary.org/obo/GAZ_00002713"/>
        <obo:IAO_0000115>A forest in the Galilee region. Located near Kibbutz Parod.</obo:IAO_0000115>
        <oboInOwl:hasOBONamespace>GAZ</oboInOwl:hasOBONamespace>
        <oboInOwl:id>GAZ:00193910</oboInOwl:id>
        <rdfs:label>Parod Forest</rdfs:label>
    </owl:NamedIndividual>
    


    <!-- http://purl.obolibrary.org/obo/GAZ_00193911 -->

    <owl:NamedIndividual rdf:about="http://purl.obolibrary.org/obo/GAZ_00193911">
        <obo:RO_0001025 rdf:resource="http://purl.obolibrary.org/obo/GAZ_00002713"/>
        <obo:IAO_0000115>A forest in the Galilee region. Located near Mount Gamal.</obo:IAO_0000115>
        <oboInOwl:hasOBONamespace>GAZ</oboInOwl:hasOBONamespace>
        <oboInOwl:id>GAZ:00193911</oboInOwl:id>
        <rdfs:label>Ahihud Forest</rdfs:label>
    </owl:NamedIndividual>
    


    <!-- http://purl.obolibrary.org/obo/GAZ_00193912 -->

    <owl:NamedIndividual rdf:about="http://purl.obolibrary.org/obo/GAZ_00193912">
        <obo:RO_0001025 rdf:resource="http://purl.obolibrary.org/obo/GAZ_00002713"/>
        <obo:IAO_0000115>A forest. Located near Amikam.</obo:IAO_0000115>
        <oboInOwl:hasOBONamespace>GAZ</oboInOwl:hasOBONamespace>
        <oboInOwl:id>GAZ:00193912</oboInOwl:id>
        <rdfs:label>Mount Hurshan Forest</rdfs:label>
    </owl:NamedIndividual>
    


    <!-- http://purl.obolibrary.org/obo/GAZ_00193913 -->

    <owl:NamedIndividual rdf:about="http://purl.obolibrary.org/obo/GAZ_00193913">
        <obo:RO_0001025 rdf:resource="http://purl.obolibrary.org/obo/GAZ_00002713"/>
        <obo:IAO_0000115>A forest.</obo:IAO_0000115>
        <oboInOwl:hasOBONamespace>GAZ</oboInOwl:hasOBONamespace>
        <oboInOwl:id>GAZ:00193913</oboInOwl:id>
        <rdfs:label>Hadera Forest</rdfs:label>
    </owl:NamedIndividual>
    


    <!-- http://purl.obolibrary.org/obo/GAZ_00193914 -->

    <owl:NamedIndividual rdf:about="http://purl.obolibrary.org/obo/GAZ_00193914">
        <obo:RO_0001025 rdf:resource="http://purl.obolibrary.org/obo/GAZ_00002713"/>
        <obo:IAO_0000115>A forest.</obo:IAO_0000115>
        <oboInOwl:hasOBONamespace>GAZ</oboInOwl:hasOBONamespace>
        <oboInOwl:id>GAZ:00193914</oboInOwl:id>
        <rdfs:label>Mount Shehumit (Har Nahash) Forest</rdfs:label>
    </owl:NamedIndividual>
    


    <!-- http://purl.obolibrary.org/obo/GAZ_00193915 -->

    <owl:NamedIndividual rdf:about="http://purl.obolibrary.org/obo/GAZ_00193915">
        <obo:RO_0001025 rdf:resource="http://purl.obolibrary.org/obo/GAZ_00002713"/>
        <obo:IAO_0000115>A forest.</obo:IAO_0000115>
        <oboInOwl:hasOBONamespace>GAZ</oboInOwl:hasOBONamespace>
        <oboInOwl:id>GAZ:00193915</oboInOwl:id>
        <rdfs:label>Irron Forest</rdfs:label>
    </owl:NamedIndividual>
    


    <!-- http://purl.obolibrary.org/obo/GAZ_00193916 -->

    <owl:NamedIndividual rdf:about="http://purl.obolibrary.org/obo/GAZ_00193916">
        <obo:RO_0001025 rdf:resource="http://purl.obolibrary.org/obo/GAZ_00002714"/>
        <obo:IAO_0000115>A forest.</obo:IAO_0000115>
        <oboInOwl:hasOBONamespace>GAZ</oboInOwl:hasOBONamespace>
        <oboInOwl:id>GAZ:00193916</oboInOwl:id>
        <rdfs:label>Hulda Forest</rdfs:label>
    </owl:NamedIndividual>
    


    <!-- http://purl.obolibrary.org/obo/GAZ_00193917 -->

    <owl:NamedIndividual rdf:about="http://purl.obolibrary.org/obo/GAZ_00193917">
        <obo:RO_0001025 rdf:resource="http://purl.obolibrary.org/obo/GAZ_00002714"/>
        <obo:IAO_0000115>A forest. Located near Tzora.</obo:IAO_0000115>
        <oboInOwl:hasOBONamespace>GAZ</oboInOwl:hasOBONamespace>
        <oboInOwl:id>GAZ:00193917</oboInOwl:id>
        <rdfs:label>Tzora Forest</rdfs:label>
    </owl:NamedIndividual>
    


    <!-- http://purl.obolibrary.org/obo/GAZ_00193918 -->

    <owl:NamedIndividual rdf:about="http://purl.obolibrary.org/obo/GAZ_00193918">
        <obo:RO_0001025 rdf:resource="http://purl.obolibrary.org/obo/GAZ_00002714"/>
        <obo:IAO_0000115>A forest. Located east of Ben Shemen Youth Village.</obo:IAO_0000115>
        <oboInOwl:hasOBONamespace>GAZ</oboInOwl:hasOBONamespace>
        <oboInOwl:id>GAZ:00193918</oboInOwl:id>
        <rdfs:label>Ben Shemen Forest</rdfs:label>
    </owl:NamedIndividual>
    


    <!-- http://purl.obolibrary.org/obo/GAZ_00193919 -->

    <owl:NamedIndividual rdf:about="http://purl.obolibrary.org/obo/GAZ_00193919">
        <obo:RO_0001025 rdf:resource="http://purl.obolibrary.org/obo/GAZ_00078176"/>
        <obo:IAO_0000115>A forest located below East Talpiot promenade.</obo:IAO_0000115>
        <oboInOwl:hasOBONamespace>GAZ</oboInOwl:hasOBONamespace>
        <oboInOwl:id>GAZ:00193919</oboInOwl:id>
        <rdfs:label>Peace Forest</rdfs:label>
    </owl:NamedIndividual>
    


    <!-- http://purl.obolibrary.org/obo/GAZ_00193920 -->

    <owl:NamedIndividual rdf:about="http://purl.obolibrary.org/obo/GAZ_00193920">
        <obo:RO_0001025 rdf:resource="http://purl.obolibrary.org/obo/GAZ_00078176"/>
        <obo:IAO_0000115>A forest on the outskirts of Jerusalem, Israel. It is located on the western edge of Eshtaol Forest near Beit Meir.</obo:IAO_0000115>
        <oboInOwl:hasOBONamespace>GAZ</oboInOwl:hasOBONamespace>
        <oboInOwl:id>GAZ:00193920</oboInOwl:id>
        <rdfs:label>Forest of the Martyrs</rdfs:label>
    </owl:NamedIndividual>
    


    <!-- http://purl.obolibrary.org/obo/GAZ_00193921 -->

    <owl:NamedIndividual rdf:about="http://purl.obolibrary.org/obo/GAZ_00193921">
        <obo:RO_0001025 rdf:resource="http://purl.obolibrary.org/obo/GAZ_00193927"/>
        <obo:IAO_0000115>A forest in the Gilo district.</obo:IAO_0000115>
        <oboInOwl:hasOBONamespace>GAZ</oboInOwl:hasOBONamespace>
        <oboInOwl:id>GAZ:00193921</oboInOwl:id>
        <rdfs:label>Gilo Forest</rdfs:label>
    </owl:NamedIndividual>
    


    <!-- http://purl.obolibrary.org/obo/GAZ_00193922 -->

    <owl:NamedIndividual rdf:about="http://purl.obolibrary.org/obo/GAZ_00193922">
        <obo:RO_0001025 rdf:resource="http://purl.obolibrary.org/obo/GAZ_00078176"/>
        <obo:IAO_0000115>A forest located between Ramot neighborhood and Shu&apos;afat.</obo:IAO_0000115>
        <oboInOwl:hasOBONamespace>GAZ</oboInOwl:hasOBONamespace>
        <oboInOwl:id>GAZ:00193922</oboInOwl:id>
        <rdfs:label>Ramot Forest</rdfs:label>
    </owl:NamedIndividual>
    


    <!-- http://purl.obolibrary.org/obo/GAZ_00193923 -->

    <owl:NamedIndividual rdf:about="http://purl.obolibrary.org/obo/GAZ_00193923">
        <obo:RO_0001025 rdf:resource="http://purl.obolibrary.org/obo/GAZ_00078176"/>
        <obo:IAO_0000115>A pine forest located in the Judean Mountains west of Jerusalem. It is surrounded by the Jerusalem neighborhoods Beit HaKerem, Yefe Nof, Ein Kerem, Har Nof, Givat Shaul, and a moshav, Beit Zeit. The forest was planted during the 1950s.</obo:IAO_0000115>
        <oboInOwl:hasOBONamespace>GAZ</oboInOwl:hasOBONamespace>
        <oboInOwl:id>GAZ:00193923</oboInOwl:id>
        <rdfs:label>Jerusalem Forest</rdfs:label>
    </owl:NamedIndividual>
    


    <!-- http://purl.obolibrary.org/obo/GAZ_00193924 -->

    <owl:NamedIndividual rdf:about="http://purl.obolibrary.org/obo/GAZ_00193924">
        <obo:RO_0001025 rdf:resource="http://purl.obolibrary.org/obo/GAZ_00078176"/>
        <obo:IAO_0000115>A forest located in the Judean Hills near Aminadav.</obo:IAO_0000115>
        <oboInOwl:hasOBONamespace>GAZ</oboInOwl:hasOBONamespace>
        <oboInOwl:id>GAZ:00193924</oboInOwl:id>
        <rdfs:label>Aminadav Forest</rdfs:label>
    </owl:NamedIndividual>
    


    <!-- http://purl.obolibrary.org/obo/GAZ_00193925 -->

    <owl:NamedIndividual rdf:about="http://purl.obolibrary.org/obo/GAZ_00193925">
        <obo:RO_0001025 rdf:resource="http://purl.obolibrary.org/obo/GAZ_00078176"/>
        <obo:IAO_0000115>A forest in Israel, located north of Beit Shemesh and near Ta&apos;oz and Neve Shalom.</obo:IAO_0000115>
        <oboInOwl:hasOBONamespace>GAZ</oboInOwl:hasOBONamespace>
        <oboInOwl:id>GAZ:00193925</oboInOwl:id>
        <rdfs:label>Eshtaol Forest</rdfs:label>
    </owl:NamedIndividual>
    


    <!-- http://purl.obolibrary.org/obo/GAZ_00193926 -->

    <owl:NamedIndividual rdf:about="http://purl.obolibrary.org/obo/GAZ_00193926">
        <obo:RO_0001025 rdf:resource="http://purl.obolibrary.org/obo/GAZ_00078176"/>
        <obo:IAO_0000115>A forest.</obo:IAO_0000115>
        <oboInOwl:hasOBONamespace>GAZ</oboInOwl:hasOBONamespace>
        <oboInOwl:id>GAZ:00193926</oboInOwl:id>
        <rdfs:label>Canada Forest</rdfs:label>
    </owl:NamedIndividual>
    


    <!-- http://purl.obolibrary.org/obo/GAZ_00193927 -->

    <owl:NamedIndividual rdf:about="http://purl.obolibrary.org/obo/GAZ_00193927">
        <obo:RO_0001025 rdf:resource="http://purl.obolibrary.org/obo/GAZ_00003782"/>
        <obo:IAO_0000115>A neighborhood in Jerusalem, located in the south of greater Jerusalem.</obo:IAO_0000115>
        <oboInOwl:hasOBONamespace>GAZ</oboInOwl:hasOBONamespace>
        <oboInOwl:id>GAZ:00193927</oboInOwl:id>
        <rdfs:label>Gilo</rdfs:label>
    </owl:NamedIndividual>
    


    <!-- http://purl.obolibrary.org/obo/GAZ_00193928 -->

    <owl:NamedIndividual rdf:about="http://purl.obolibrary.org/obo/GAZ_00193928">
        <obo:RO_0001025 rdf:resource="http://purl.obolibrary.org/obo/GAZ_00002713"/>
        <obo:IAO_0000115>A geologic formation in Israel, located on the coast of the Mediterranean Sea, in the Western Galilee near the border with Lebanon. It is a white chalk cliff face which opens up into spectacular grottos.</obo:IAO_0000115>
        <oboInOwl:hasOBONamespace>GAZ</oboInOwl:hasOBONamespace>
        <oboInOwl:id>GAZ:00193928</oboInOwl:id>
        <rdfs:label>Rosh HaNikra Grottoes</rdfs:label>
    </owl:NamedIndividual>
    


    <!-- http://purl.obolibrary.org/obo/GAZ_00193929 -->

    <owl:NamedIndividual rdf:about="http://purl.obolibrary.org/obo/GAZ_00193929">
        <obo:RO_0001025 rdf:resource="http://purl.obolibrary.org/obo/GAZ_00057704"/>
        <obo:IAO_0000115>A National Park in the Negev desert of Israel, located approximately 30km north of Eilat.</obo:IAO_0000115>
        <oboInOwl:hasOBONamespace>GAZ</oboInOwl:hasOBONamespace>
        <oboInOwl:id>GAZ:00193929</oboInOwl:id>
        <rdfs:label>Timna Valley Park</rdfs:label>
    </owl:NamedIndividual>
    


    <!-- http://purl.obolibrary.org/obo/GAZ_00193930 -->

    <owl:NamedIndividual rdf:about="http://purl.obolibrary.org/obo/GAZ_00193930">
        <obo:RO_0001025 rdf:resource="http://purl.obolibrary.org/obo/GAZ_00078270"/>
        <obo:IAO_0000115>A public park in Tel Aviv, Israel, lying at the back of the Tel Aviv Performing Arts Center.</obo:IAO_0000115>
        <oboInOwl:hasOBONamespace>GAZ</oboInOwl:hasOBONamespace>
        <oboInOwl:id>GAZ:00193930</oboInOwl:id>
        <rdfs:label>Dubnow Park</rdfs:label>
    </owl:NamedIndividual>
    


    <!-- http://purl.obolibrary.org/obo/GAZ_00193931 -->

    <owl:NamedIndividual rdf:about="http://purl.obolibrary.org/obo/GAZ_00193931">
        <obo:RO_0001025 rdf:resource="http://purl.obolibrary.org/obo/GAZ_00078350"/>
        <obo:IAO_0000115>An open space of 260 dunams in the heart of Jerusalem, Israel, on the edge of the Givat Mordechai neighborhood.</obo:IAO_0000115>
        <oboInOwl:hasOBONamespace>GAZ</oboInOwl:hasOBONamespace>
        <oboInOwl:id>GAZ:00193931</oboInOwl:id>
        <rdfs:label>Pri Har Valley</rdfs:label>
    </owl:NamedIndividual>
    


    <!-- http://purl.obolibrary.org/obo/GAZ_00193932 -->

    <owl:NamedIndividual rdf:about="http://purl.obolibrary.org/obo/GAZ_00193932">
        <obo:RO_0001025 rdf:resource="http://purl.obolibrary.org/obo/GAZ_00078270"/>
        <obo:IAO_0000115>A public park, lying between King George Street and Tchernichovsky Street in central Tel Aviv, Israel. Established 1944-03-10.</obo:IAO_0000115>
        <oboInOwl:hasOBONamespace>GAZ</oboInOwl:hasOBONamespace>
        <oboInOwl:id>GAZ:00193932</oboInOwl:id>
        <rdfs:label>Meir Park</rdfs:label>
    </owl:NamedIndividual>
    


    <!-- http://purl.obolibrary.org/obo/GAZ_00193933 -->

    <owl:NamedIndividual rdf:about="http://purl.obolibrary.org/obo/GAZ_00193933">
        <obo:RO_0001025 rdf:resource="http://purl.obolibrary.org/obo/GAZ_00078277"/>
        <obo:IAO_0000115>A large urban park in Ramat Gan, Israel.</obo:IAO_0000115>
        <oboInOwl:hasOBONamespace>GAZ</oboInOwl:hasOBONamespace>
        <oboInOwl:id>GAZ:00193933</oboInOwl:id>
        <rdfs:label>The National Park</rdfs:label>
    </owl:NamedIndividual>
    


    <!-- http://purl.obolibrary.org/obo/GAZ_00193934 -->

    <owl:NamedIndividual rdf:about="http://purl.obolibrary.org/obo/GAZ_00193934">
        <obo:RO_0001025 rdf:resource="http://purl.obolibrary.org/obo/GAZ_00002711"/>
        <obo:IAO_0000115>A nature park in northern Israel, covering 4.5 km at the southern end of Mount Carmel between Zichron Ya&apos;akov to the north and Binyamina to the south.</obo:IAO_0000115>
        <oboInOwl:hasOBONamespace>GAZ</oboInOwl:hasOBONamespace>
        <oboInOwl:id>GAZ:00193934</oboInOwl:id>
        <rdfs:label>Ramat HaNadiv</rdfs:label>
    </owl:NamedIndividual>
    


    <!-- http://purl.obolibrary.org/obo/GAZ_00193935 -->

    <owl:NamedIndividual rdf:about="http://purl.obolibrary.org/obo/GAZ_00193935">
        <obo:RO_0001025 rdf:resource="http://purl.obolibrary.org/obo/GAZ_00002714"/>
        <obo:IAO_0000115>A large underground limestone cave located near Ramla, Israel.</obo:IAO_0000115>
        <oboInOwl:hasOBONamespace>GAZ</oboInOwl:hasOBONamespace>
        <oboInOwl:id>GAZ:00193935</oboInOwl:id>
        <rdfs:label>Ayalon Cave</rdfs:label>
    </owl:NamedIndividual>
    


    <!-- http://purl.obolibrary.org/obo/GAZ_00193936 -->

    <owl:NamedIndividual rdf:about="http://purl.obolibrary.org/obo/GAZ_00193936">
        <obo:RO_0001025 rdf:resource="http://purl.obolibrary.org/obo/GAZ_00193814"/>
        <obo:IAO_0000115>An Israeli limestone cave locality of the Wadi Kebara, situated at 60 - 65 m ASL on the western escarpment of the Carmel Range, some 10 km north-east of Caesarea.</obo:IAO_0000115>
        <oboInOwl:hasOBONamespace>GAZ</oboInOwl:hasOBONamespace>
        <oboInOwl:id>GAZ:00193936</oboInOwl:id>
        <rdfs:label>Kebara Cave</rdfs:label>
    </owl:NamedIndividual>
    


    <!-- http://purl.obolibrary.org/obo/GAZ_00193937 -->

    <owl:NamedIndividual rdf:about="http://purl.obolibrary.org/obo/GAZ_00193937">
        <obo:IAO_0000115>A crater lake (maar) in the northeastern Golan Heights, near Mount Hermon. The only sources of the lake are rain water and an underground spring.</obo:IAO_0000115>
        <oboInOwl:hasOBONamespace>GAZ</oboInOwl:hasOBONamespace>
        <oboInOwl:id>GAZ:00193937</oboInOwl:id>
        <rdfs:label>Birkat Ram</rdfs:label>
    </owl:NamedIndividual>
    


    <!-- http://purl.obolibrary.org/obo/GAZ_00193938 -->

    <owl:NamedIndividual rdf:about="http://purl.obolibrary.org/obo/GAZ_00193938">
        <obo:RO_0001025 rdf:resource="http://purl.obolibrary.org/obo/GAZ_00000670"/>
        <obo:IAO_0000115>A saline desert lake located on the edge of the Red Sea, about 18 km south of Eilat in the Sinai Peninsula, Israel, very close to the border with Egypt.</obo:IAO_0000115>
        <oboInOwl:hasOBONamespace>GAZ</oboInOwl:hasOBONamespace>
        <oboInOwl:id>GAZ:00193938</oboInOwl:id>
        <rdfs:label>Solar Lake</rdfs:label>
    </owl:NamedIndividual>
    


    <!-- http://purl.obolibrary.org/obo/GAZ_00193939 -->

    <owl:NamedIndividual rdf:about="http://purl.obolibrary.org/obo/GAZ_00193939">
        <obo:RO_0001025 rdf:resource="http://purl.obolibrary.org/obo/GAZ_00002476"/>
        <obo:IAO_0000115>A emountain range of the Judea region upon which Jerusalem and several other cities are located. Running generally north-south, the mountains extend both to the west and east of Jerusalem, the southern end known as Mount Hebron. Other important cities in the mountain range are Hebron, Bethlehem and Ramallah. The range forms a natural division between the Shephelah coastal plains to the west and the Jordan Rift Valley to the east, as well as causing the rain shadow responsible for the Judean desert.</obo:IAO_0000115>
        <oboInOwl:hasOBONamespace>GAZ</oboInOwl:hasOBONamespace>
        <oboInOwl:id>GAZ:00193939</oboInOwl:id>
        <rdfs:label>Judean Mountains</rdfs:label>
    </owl:NamedIndividual>
    


    <!-- http://purl.obolibrary.org/obo/GAZ_00193940 -->

    <owl:NamedIndividual rdf:about="http://purl.obolibrary.org/obo/GAZ_00193940">
        <obo:RO_0001025 rdf:resource="http://purl.obolibrary.org/obo/GAZ_00002476"/>
        <obo:IAO_0000115>A small river in north-western Israel.</obo:IAO_0000115>
        <oboInOwl:hasOBONamespace>GAZ</oboInOwl:hasOBONamespace>
        <oboInOwl:id>GAZ:00193940</oboInOwl:id>
        <rdfs:label>Na&apos;aman River</rdfs:label>
    </owl:NamedIndividual>
    


    <!-- http://purl.obolibrary.org/obo/GAZ_00193941 -->

    <owl:NamedIndividual rdf:about="http://purl.obolibrary.org/obo/GAZ_00193941">
        <obo:RO_0001025 rdf:resource="http://purl.obolibrary.org/obo/GAZ_00002713"/>
        <oboInOwl:hasOBONamespace>GAZ</oboInOwl:hasOBONamespace>
        <oboInOwl:id>GAZ:00193941</oboInOwl:id>
        <rdfs:label>Beit She&apos;an Valley</rdfs:label>
    </owl:NamedIndividual>
    


    <!-- http://purl.obolibrary.org/obo/GAZ_00193942 -->

    <owl:NamedIndividual rdf:about="http://purl.obolibrary.org/obo/GAZ_00193942">
        <obo:RO_0001025 rdf:resource="http://purl.obolibrary.org/obo/GAZ_00193941"/>
        <obo:IAO_0000115>A spring situated 4 km north-east of Bet She&apos;an, and to the east of the Kibbutz at Hamadia. It is one of the most important sources of water in the Bet She&apos;an valley.</obo:IAO_0000115>
        <oboInOwl:hasOBONamespace>GAZ</oboInOwl:hasOBONamespace>
        <oboInOwl:id>GAZ:00193942</oboInOwl:id>
        <rdfs:label>Ein Hoga</rdfs:label>
    </owl:NamedIndividual>
    


    <!-- http://purl.obolibrary.org/obo/GAZ_00193943 -->

    <owl:NamedIndividual rdf:about="http://purl.obolibrary.org/obo/GAZ_00193943">
        <obo:RO_0001025 rdf:resource="http://purl.obolibrary.org/obo/GAZ_00002713"/>
        <obo:IAO_0000115>A small river in the North District of Israel. It passes through the town of Nahariya before discharging to the Mediterranean Sea. The river runs through the main street of Nahariya.</obo:IAO_0000115>
        <oboInOwl:hasOBONamespace>GAZ</oboInOwl:hasOBONamespace>
        <oboInOwl:id>GAZ:00193943</oboInOwl:id>
        <rdfs:label>Ga&apos;aton River</rdfs:label>
    </owl:NamedIndividual>
    


    <!-- http://purl.obolibrary.org/obo/GAZ_00193947 -->

    <owl:NamedIndividual rdf:about="http://purl.obolibrary.org/obo/GAZ_00193947">
        <obo:RO_0001025 rdf:resource="http://purl.obolibrary.org/obo/GAZ_00193939"/>
        <obo:IAO_0000115>A river in the Judean Hills.</obo:IAO_0000115>
        <oboInOwl:hasOBONamespace>GAZ</oboInOwl:hasOBONamespace>
        <oboInOwl:id>GAZ:00193947</oboInOwl:id>
        <rdfs:label>Nahal Sorek</rdfs:label>
    </owl:NamedIndividual>
    


    <!-- http://purl.obolibrary.org/obo/GAZ_00193948 -->

    <owl:NamedIndividual rdf:about="http://purl.obolibrary.org/obo/GAZ_00193948">
        <obo:RO_0001025 rdf:resource="http://purl.obolibrary.org/obo/GAZ_00078379"/>
        <obo:IAO_0000115>A spring in Acre.</obo:IAO_0000115>
        <oboInOwl:hasOBONamespace>GAZ</oboInOwl:hasOBONamespace>
        <oboInOwl:id>GAZ:00193948</oboInOwl:id>
        <rdfs:label>Aynu&apos;l-Baqar?</rdfs:label>
    </owl:NamedIndividual>
    


    <!-- http://purl.obolibrary.org/obo/GAZ_00193949 -->

    <owl:NamedIndividual rdf:about="http://purl.obolibrary.org/obo/GAZ_00193949">
        <obo:RO_0001025 rdf:resource="http://purl.obolibrary.org/obo/GAZ_00057703"/>
        <obo:IAO_0000115>A wadi and canyon situated in the Judean Desert, Israel, near Masada, descending to the Dead Sea.</obo:IAO_0000115>
        <oboInOwl:hasOBONamespace>GAZ</oboInOwl:hasOBONamespace>
        <oboInOwl:id>GAZ:00193949</oboInOwl:id>
        <rdfs:label>Tze&apos;elim Stream</rdfs:label>
    </owl:NamedIndividual>
    


    <!-- http://purl.obolibrary.org/obo/GAZ_00193950 -->

    <owl:NamedIndividual rdf:about="http://purl.obolibrary.org/obo/GAZ_00193950">
        <obo:RO_0001025 rdf:resource="http://purl.obolibrary.org/obo/GAZ_00193949"/>
        <obo:IAO_0000115>A headspring located in the middle of the Tze&apos;elim canyon.</obo:IAO_0000115>
        <oboInOwl:hasOBONamespace>GAZ</oboInOwl:hasOBONamespace>
        <oboInOwl:id>GAZ:00193950</oboInOwl:id>
        <rdfs:label>Ein Namer</rdfs:label>
    </owl:NamedIndividual>
    


    <!-- http://purl.obolibrary.org/obo/GAZ_00193951 -->

    <owl:NamedIndividual rdf:about="http://purl.obolibrary.org/obo/GAZ_00193951">
        <obo:RO_0001025 rdf:resource="http://purl.obolibrary.org/obo/GAZ_00044915"/>
        <obo:IAO_0000115>A large spit of land which now separates the North and the South basins of the Dead Sea. Entirely located in Jordan.</obo:IAO_0000115>
        <oboInOwl:hasOBONamespace>GAZ</oboInOwl:hasOBONamespace>
        <oboInOwl:id>GAZ:00193951</oboInOwl:id>
        <rdfs:label>Lisan Peninsula</rdfs:label>
    </owl:NamedIndividual>
    


    <!-- http://purl.obolibrary.org/obo/GAZ_00193952 -->

    <owl:NamedIndividual rdf:about="http://purl.obolibrary.org/obo/GAZ_00193952">
        <obo:RO_0001025 rdf:resource="http://purl.obolibrary.org/obo/GAZ_00002476"/>
        <obo:IAO_0000115>The narrow coastal plain along Israel&apos;s Mediterranean Sea coast which houses 70% of the country&apos;s population. The plain extends 187 km north to south and is divided into a number of areas; the Plain of Zebulun (north of Haifa), Hof HaCarmel (from Haifa to Mount Carmel), the Sharon plain (from Mount Carmel to Tel Aviv), and the Plain of Judea (from Tel Aviv to Zikim).</obo:IAO_0000115>
        <oboInOwl:hasOBONamespace>GAZ</oboInOwl:hasOBONamespace>
        <oboInOwl:id>GAZ:00193952</oboInOwl:id>
        <rdfs:label>Israeli Coastal Plain</rdfs:label>
    </owl:NamedIndividual>
    


    <!-- http://purl.obolibrary.org/obo/GAZ_00193953 -->

    <owl:NamedIndividual rdf:about="http://purl.obolibrary.org/obo/GAZ_00193953">
        <obo:RO_0001025 rdf:resource="http://purl.obolibrary.org/obo/GAZ_00193952"/>
        <obo:IAO_0000115>The region of the Coastal Plain that extends south to the Gaza Strip.</obo:IAO_0000115>
        <oboInOwl:hasOBONamespace>GAZ</oboInOwl:hasOBONamespace>
        <oboInOwl:id>GAZ:00193953</oboInOwl:id>
        <rdfs:label>Southern Coastal Plain</rdfs:label>
    </owl:NamedIndividual>
    


    <!-- http://purl.obolibrary.org/obo/GAZ_00193954 -->

    <owl:NamedIndividual rdf:about="http://purl.obolibrary.org/obo/GAZ_00193954">
        <obo:RO_0001025 rdf:resource="http://purl.obolibrary.org/obo/GAZ_00193952"/>
        <obo:IAO_0000115>The region of the Coastal Plain that stretches from Rosh HaNikra in the far North, down to Israel&apos;s third-largest city, Haifa.</obo:IAO_0000115>
        <oboInOwl:hasOBONamespace>GAZ</oboInOwl:hasOBONamespace>
        <oboInOwl:id>GAZ:00193954</oboInOwl:id>
        <rdfs:label>Plain of Zebulun</rdfs:label>
    </owl:NamedIndividual>
    


    <!-- http://purl.obolibrary.org/obo/GAZ_00193955 -->

    <owl:NamedIndividual rdf:about="http://purl.obolibrary.org/obo/GAZ_00193955">
        <obo:RO_0001025 rdf:resource="http://purl.obolibrary.org/obo/GAZ_00193952"/>
        <obo:IAO_0000115>The region of the Coastal Plain covers the area from Haifa down to the town of Zikhron Ya&apos;aqov, the coast nearby Mount Carmel.</obo:IAO_0000115>
        <oboInOwl:hasOBONamespace>GAZ</oboInOwl:hasOBONamespace>
        <oboInOwl:id>GAZ:00193955</oboInOwl:id>
        <rdfs:label>Hof HaCarmel</rdfs:label>
    </owl:NamedIndividual>
    


    <!-- http://purl.obolibrary.org/obo/GAZ_00193956 -->

    <owl:NamedIndividual rdf:about="http://purl.obolibrary.org/obo/GAZ_00193956">
        <obo:RO_0001025 rdf:resource="http://purl.obolibrary.org/obo/GAZ_00193952"/>
        <obo:IAO_0000115>The region of the Coastal Plain running from Zikhron Ya&apos;aqov to Tel Aviv&apos;s Yarkon River.</obo:IAO_0000115>
        <oboInOwl:hasOBONamespace>GAZ</oboInOwl:hasOBONamespace>
        <oboInOwl:id>GAZ:00193956</oboInOwl:id>
        <rdfs:label>Sharon Plain</rdfs:label>
    </owl:NamedIndividual>
    


    <!-- http://purl.obolibrary.org/obo/GAZ_00193957 -->

    <owl:NamedIndividual rdf:about="http://purl.obolibrary.org/obo/GAZ_00193957">
        <obo:RO_0001025 rdf:resource="http://purl.obolibrary.org/obo/GAZ_00193952"/>
        <obo:IAO_0000115>The region of the Coastal Plain running from Northern Tel Aviv&apos;s Yarkon River to Nakhal Shikma.</obo:IAO_0000115>
        <oboInOwl:hasOBONamespace>GAZ</oboInOwl:hasOBONamespace>
        <oboInOwl:id>GAZ:00193957</oboInOwl:id>
        <rdfs:label>Central Coastal Plain</rdfs:label>
    </owl:NamedIndividual>
    


    <!-- http://purl.obolibrary.org/obo/GAZ_00193958 -->

    <owl:NamedIndividual rdf:about="http://purl.obolibrary.org/obo/GAZ_00193958">
        <obo:RO_0001025 rdf:resource="http://purl.obolibrary.org/obo/GAZ_00193953"/>
        <obo:IAO_0000115>The N part of the Southern Coastal Plain.</obo:IAO_0000115>
        <oboInOwl:hasOBONamespace>GAZ</oboInOwl:hasOBONamespace>
        <oboInOwl:id>GAZ:00193958</oboInOwl:id>
        <rdfs:label>Besor Region</rdfs:label>
    </owl:NamedIndividual>
    


    <!-- http://purl.obolibrary.org/obo/GAZ_00193959 -->

    <owl:NamedIndividual rdf:about="http://purl.obolibrary.org/obo/GAZ_00193959">
        <obo:RO_0001025 rdf:resource="http://purl.obolibrary.org/obo/GAZ_00193953"/>
        <obo:IAO_0000115>The S part of the Southern Coastal Plain.</obo:IAO_0000115>
        <oboInOwl:hasOBONamespace>GAZ</oboInOwl:hasOBONamespace>
        <oboInOwl:id>GAZ:00193959</oboInOwl:id>
        <rdfs:label>Agur-Halutsa Region</rdfs:label>
    </owl:NamedIndividual>
    


    <!-- http://purl.obolibrary.org/obo/GAZ_00230322 -->

    <owl:NamedIndividual rdf:about="http://purl.obolibrary.org/obo/GAZ_00230322">
        <obo:RO_0001025 rdf:resource="http://purl.obolibrary.org/obo/GAZ_00000670"/>
        <obo:IAO_0000115>An oasis valley in the southern Sinai region of Egypt.</obo:IAO_0000115>
        <oboInOwl:hasOBONamespace>GAZ</oboInOwl:hasOBONamespace>
        <oboInOwl:id>GAZ:00230322</oboInOwl:id>
        <rdfs:label>Wadi Faran</rdfs:label>
    </owl:NamedIndividual>
    


    <!-- http://purl.obolibrary.org/obo/GAZ_00241992 -->

    <owl:NamedIndividual rdf:about="http://purl.obolibrary.org/obo/GAZ_00241992">
        <obo:RO_0001025 rdf:resource="http://purl.obolibrary.org/obo/GAZ_00066423"/>
        <obo:IAO_0000115>An administrative region (kism) of North Sinai Governorate.</obo:IAO_0000115>
        <oboInOwl:hasOBONamespace>GAZ</oboInOwl:hasOBONamespace>
        <oboInOwl:id>GAZ:00241992</oboInOwl:id>
        <rdfs:label>Kism Al &apos;Arish First</rdfs:label>
    </owl:NamedIndividual>
    


    <!-- http://purl.obolibrary.org/obo/GAZ_00241993 -->

    <owl:NamedIndividual rdf:about="http://purl.obolibrary.org/obo/GAZ_00241993">
        <obo:RO_0001025 rdf:resource="http://purl.obolibrary.org/obo/GAZ_00066423"/>
        <obo:IAO_0000115>An administrative region (kism) of North Sinai Governorate.</obo:IAO_0000115>
        <oboInOwl:hasOBONamespace>GAZ</oboInOwl:hasOBONamespace>
        <oboInOwl:id>GAZ:00241993</oboInOwl:id>
        <rdfs:label>Kism Al &apos;Arish Second</rdfs:label>
    </owl:NamedIndividual>
    


    <!-- http://purl.obolibrary.org/obo/GAZ_00241994 -->

    <owl:NamedIndividual rdf:about="http://purl.obolibrary.org/obo/GAZ_00241994">
        <obo:RO_0001025 rdf:resource="http://purl.obolibrary.org/obo/GAZ_00066423"/>
        <obo:IAO_0000115>An administrative region (kism) of North Sinai Governorate.</obo:IAO_0000115>
        <oboInOwl:hasOBONamespace>GAZ</oboInOwl:hasOBONamespace>
        <oboInOwl:id>GAZ:00241994</oboInOwl:id>
        <rdfs:label>Kism Al &apos;Arish Third</rdfs:label>
    </owl:NamedIndividual>
    


    <!-- http://purl.obolibrary.org/obo/GAZ_00241995 -->

    <owl:NamedIndividual rdf:about="http://purl.obolibrary.org/obo/GAZ_00241995">
        <obo:RO_0001025 rdf:resource="http://purl.obolibrary.org/obo/GAZ_00066423"/>
        <obo:IAO_0000115>An administrative region (kism) of North Sinai Governorate.</obo:IAO_0000115>
        <oboInOwl:hasOBONamespace>GAZ</oboInOwl:hasOBONamespace>
        <oboInOwl:id>GAZ:00241995</oboInOwl:id>
        <rdfs:label>Kism Al &apos;Arish Fourth</rdfs:label>
    </owl:NamedIndividual>
    


    <!-- http://purl.obolibrary.org/obo/GAZ_00241996 -->

    <owl:NamedIndividual rdf:about="http://purl.obolibrary.org/obo/GAZ_00241996">
        <obo:RO_0001025 rdf:resource="http://purl.obolibrary.org/obo/GAZ_00000669"/>
        <obo:IAO_0000115>An administrative region (markaz) of North Sinai Governorate.</obo:IAO_0000115>
        <oboInOwl:hasOBONamespace>GAZ</oboInOwl:hasOBONamespace>
        <oboInOwl:id>GAZ:00241996</oboInOwl:id>
        <rdfs:label>Al Qusaymah Region</rdfs:label>
    </owl:NamedIndividual>
    


    <!-- http://purl.obolibrary.org/obo/GAZ_00241997 -->

    <owl:NamedIndividual rdf:about="http://purl.obolibrary.org/obo/GAZ_00241997">
        <obo:RO_0001025 rdf:resource="http://purl.obolibrary.org/obo/GAZ_00000669"/>
        <obo:IAO_0000115>An administrative region of North Sinai Governorate.</obo:IAO_0000115>
        <oboInOwl:hasOBONamespace>GAZ</oboInOwl:hasOBONamespace>
        <oboInOwl:id>GAZ:00241997</oboInOwl:id>
        <rdfs:label>Rmana Police Center</rdfs:label>
    </owl:NamedIndividual>
    


    <!-- http://purl.obolibrary.org/obo/GAZ_00248004 -->

    <owl:NamedIndividual rdf:about="http://purl.obolibrary.org/obo/GAZ_00248004">
        <obo:RO_0001025 rdf:resource="http://purl.obolibrary.org/obo/GAZ_00000669"/>
        <obo:IAO_0000115>A salt water lagoon, 90 km long and up to 24 km wide, on the Mediterranean coast of Sinai.</obo:IAO_0000115>
        <oboInOwl:hasOBONamespace>GAZ</oboInOwl:hasOBONamespace>
        <oboInOwl:id>GAZ:00248004</oboInOwl:id>
        <rdfs:label>Sabkhet el Bardawil</rdfs:label>
    </owl:NamedIndividual>
    


    <!-- http://purl.obolibrary.org/obo/GAZ_00251586 -->

    <owl:NamedIndividual rdf:about="http://purl.obolibrary.org/obo/GAZ_00251586">
        <obo:IAO_0000115>A river that rises in the hills southwest of Irbid city and drains west into the Jordan Valley, entering the Jordan River about 20 km south of Lake Tiberias.</obo:IAO_0000115>
        <oboInOwl:hasOBONamespace>GAZ</oboInOwl:hasOBONamespace>
        <oboInOwl:id>GAZ:00251586</oboInOwl:id>
        <rdfs:label>Wadi Ziglab</rdfs:label>
    </owl:NamedIndividual>
    


    <!-- http://purl.obolibrary.org/obo/GAZ_00251587 -->

    <owl:NamedIndividual rdf:about="http://purl.obolibrary.org/obo/GAZ_00251587">
        <obo:IAO_0000115>A dam. Located about 15 km south-southwest of Ajlun.</obo:IAO_0000115>
        <oboInOwl:hasOBONamespace>GAZ</oboInOwl:hasOBONamespace>
        <oboInOwl:id>GAZ:00251587</oboInOwl:id>
        <rdfs:label>KingTalal Dam</rdfs:label>
    </owl:NamedIndividual>
    


    <!-- http://purl.obolibrary.org/obo/GAZ_00251592 -->

    <owl:NamedIndividual rdf:about="http://purl.obolibrary.org/obo/GAZ_00251592">
        <obo:IAO_0000115>A dam.</obo:IAO_0000115>
        <oboInOwl:hasOBONamespace>GAZ</oboInOwl:hasOBONamespace>
        <oboInOwl:id>GAZ:00251592</oboInOwl:id>
        <rdfs:label>Kafrein Dam</rdfs:label>
    </owl:NamedIndividual>
    


    <!-- http://purl.obolibrary.org/obo/GAZ_00251593 -->

    <owl:NamedIndividual rdf:about="http://purl.obolibrary.org/obo/GAZ_00251593">
        <obo:IAO_0000115>A dam.</obo:IAO_0000115>
        <oboInOwl:hasOBONamespace>GAZ</oboInOwl:hasOBONamespace>
        <oboInOwl:id>GAZ:00251593</oboInOwl:id>
        <rdfs:label>Shu&apos;eib Dam</rdfs:label>
    </owl:NamedIndividual>
    


    <!-- http://purl.obolibrary.org/obo/GAZ_00251594 -->

    <owl:NamedIndividual rdf:about="http://purl.obolibrary.org/obo/GAZ_00251594">
        <obo:RO_0001025 rdf:resource="http://purl.obolibrary.org/obo/GAZ_00044915"/>
        <obo:IAO_0000115>A saline lake.</obo:IAO_0000115>
        <oboInOwl:hasOBONamespace>GAZ</oboInOwl:hasOBONamespace>
        <oboInOwl:id>GAZ:00251594</oboInOwl:id>
        <rdfs:label>Kibed Pool</rdfs:label>
    </owl:NamedIndividual>
    


    <!-- http://purl.obolibrary.org/obo/GAZ_00251595 -->

    <owl:NamedIndividual rdf:about="http://purl.obolibrary.org/obo/GAZ_00251595">
        <obo:IAO_0000115>A wadi. It enters Wadi Mujib from the north only a few km from the shores of the Dead Sea.</obo:IAO_0000115>
        <oboInOwl:hasOBONamespace>GAZ</oboInOwl:hasOBONamespace>
        <oboInOwl:id>GAZ:00251595</oboInOwl:id>
        <rdfs:label>Wadi Hidan</rdfs:label>
    </owl:NamedIndividual>
    


    <!-- http://purl.obolibrary.org/obo/GAZ_02000659 -->

    <owl:NamedIndividual rdf:about="http://purl.obolibrary.org/obo/GAZ_02000659">
        <obo:RO_0001025 rdf:resource="http://purl.obolibrary.org/obo/GAZ_00002714"/>
        <oboInOwl:hasOBONamespace>GAZ</oboInOwl:hasOBONamespace>
        <oboInOwl:id>GAZ:02000659</oboInOwl:id>
        <rdfs:label>Ramla Subdistrict</rdfs:label>
    </owl:NamedIndividual>
    


    <!-- http://purl.obolibrary.org/obo/GAZ_02000660 -->

    <owl:NamedIndividual rdf:about="http://purl.obolibrary.org/obo/GAZ_02000660">
        <obo:RO_0001025 rdf:resource="http://purl.obolibrary.org/obo/GAZ_00002714"/>
        <oboInOwl:hasOBONamespace>GAZ</oboInOwl:hasOBONamespace>
        <oboInOwl:id>GAZ:02000660</oboInOwl:id>
        <rdfs:label>Petah Tiqwa Subdistrict</rdfs:label>
    </owl:NamedIndividual>
    


    <!-- http://purl.obolibrary.org/obo/GAZ_02000661 -->

    <owl:NamedIndividual rdf:about="http://purl.obolibrary.org/obo/GAZ_02000661">
        <obo:RO_0001025 rdf:resource="http://purl.obolibrary.org/obo/GAZ_00002714"/>
        <oboInOwl:hasOBONamespace>GAZ</oboInOwl:hasOBONamespace>
        <oboInOwl:id>GAZ:02000661</oboInOwl:id>
        <rdfs:label>Rehovot Subdistrict</rdfs:label>
    </owl:NamedIndividual>
    


    <!-- http://purl.obolibrary.org/obo/GAZ_02000662 -->

    <owl:NamedIndividual rdf:about="http://purl.obolibrary.org/obo/GAZ_02000662">
        <obo:RO_0001025 rdf:resource="http://purl.obolibrary.org/obo/GAZ_00002714"/>
        <oboInOwl:hasOBONamespace>GAZ</oboInOwl:hasOBONamespace>
        <oboInOwl:id>GAZ:02000662</oboInOwl:id>
        <rdfs:label>Sharon Subdistricct</rdfs:label>
    </owl:NamedIndividual>
    


    <!-- http://purl.obolibrary.org/obo/GAZ_02000663 -->

    <owl:NamedIndividual rdf:about="http://purl.obolibrary.org/obo/GAZ_02000663">
        <obo:RO_0001025 rdf:resource="http://purl.obolibrary.org/obo/GAZ_00002713"/>
        <oboInOwl:hasOBONamespace>GAZ</oboInOwl:hasOBONamespace>
        <oboInOwl:id>GAZ:02000663</oboInOwl:id>
        <rdfs:label>Kinneret Subdistrict</rdfs:label>
    </owl:NamedIndividual>
    


    <!-- http://purl.obolibrary.org/obo/GAZ_02000664 -->

    <owl:NamedIndividual rdf:about="http://purl.obolibrary.org/obo/GAZ_02000664">
        <obo:RO_0001025 rdf:resource="http://purl.obolibrary.org/obo/GAZ_00002713"/>
        <oboInOwl:hasOBONamespace>GAZ</oboInOwl:hasOBONamespace>
        <oboInOwl:id>GAZ:02000664</oboInOwl:id>
        <rdfs:label>Akko Subdistrict</rdfs:label>
    </owl:NamedIndividual>
    


    <!-- http://purl.obolibrary.org/obo/GAZ_02000665 -->

    <owl:NamedIndividual rdf:about="http://purl.obolibrary.org/obo/GAZ_02000665">
        <obo:RO_0001025 rdf:resource="http://purl.obolibrary.org/obo/GAZ_00002713"/>
        <oboInOwl:hasOBONamespace>GAZ</oboInOwl:hasOBONamespace>
        <oboInOwl:id>GAZ:02000665</oboInOwl:id>
        <rdfs:label>Zefat Subdistrict</rdfs:label>
    </owl:NamedIndividual>
    


    <!-- http://purl.obolibrary.org/obo/GAZ_02000666 -->

    <owl:NamedIndividual rdf:about="http://purl.obolibrary.org/obo/GAZ_02000666">
        <obo:RO_0001025 rdf:resource="http://purl.obolibrary.org/obo/GAZ_00002713"/>
        <oboInOwl:hasOBONamespace>GAZ</oboInOwl:hasOBONamespace>
        <oboInOwl:id>GAZ:02000666</oboInOwl:id>
        <rdfs:label>Golan Subdistrict</rdfs:label>
    </owl:NamedIndividual>
    


    <!-- http://purl.obolibrary.org/obo/GAZ_02000667 -->

    <owl:NamedIndividual rdf:about="http://purl.obolibrary.org/obo/GAZ_02000667">
        <obo:RO_0001025 rdf:resource="http://purl.obolibrary.org/obo/GAZ_00002713"/>
        <oboInOwl:hasOBONamespace>GAZ</oboInOwl:hasOBONamespace>
        <oboInOwl:id>GAZ:02000667</oboInOwl:id>
        <rdfs:label>Yizre&apos;el Subdistrict</rdfs:label>
    </owl:NamedIndividual>
    


    <!-- http://purl.obolibrary.org/obo/GAZ_02000668 -->

    <owl:NamedIndividual rdf:about="http://purl.obolibrary.org/obo/GAZ_02000668">
        <obo:RO_0001025 rdf:resource="http://purl.obolibrary.org/obo/GAZ_00002711"/>
        <oboInOwl:hasOBONamespace>GAZ</oboInOwl:hasOBONamespace>
        <oboInOwl:id>GAZ:02000668</oboInOwl:id>
        <rdfs:label>Hadera Subdistrict</rdfs:label>
    </owl:NamedIndividual>
    


    <!-- http://purl.obolibrary.org/obo/GAZ_02000669 -->

    <owl:NamedIndividual rdf:about="http://purl.obolibrary.org/obo/GAZ_02000669">
        <obo:RO_0001025 rdf:resource="http://purl.obolibrary.org/obo/GAZ_00002711"/>
        <oboInOwl:hasOBONamespace>GAZ</oboInOwl:hasOBONamespace>
        <oboInOwl:id>GAZ:02000669</oboInOwl:id>
        <rdfs:label>Haifa Subdistrict</rdfs:label>
    </owl:NamedIndividual>
    


    <!-- http://purl.obolibrary.org/obo/GAZ_02000670 -->

    <owl:NamedIndividual rdf:about="http://purl.obolibrary.org/obo/GAZ_02000670">
        <obo:RO_0001025 rdf:resource="http://purl.obolibrary.org/obo/GAZ_00002710"/>
        <oboInOwl:hasOBONamespace>GAZ</oboInOwl:hasOBONamespace>
        <oboInOwl:id>GAZ:02000670</oboInOwl:id>
        <rdfs:label>Be&apos;er Sheva Subdistrict</rdfs:label>
    </owl:NamedIndividual>
    


    <!-- http://purl.obolibrary.org/obo/GAZ_02000671 -->

    <owl:NamedIndividual rdf:about="http://purl.obolibrary.org/obo/GAZ_02000671">
        <obo:RO_0001025 rdf:resource="http://purl.obolibrary.org/obo/GAZ_00002710"/>
        <oboInOwl:hasOBONamespace>GAZ</oboInOwl:hasOBONamespace>
        <oboInOwl:id>GAZ:02000671</oboInOwl:id>
        <rdfs:label>Ashkelon Subdistrict</rdfs:label>
    </owl:NamedIndividual>
    


    <!-- http://purl.obolibrary.org/obo/GAZ_22224105 -->

    <owl:NamedIndividual rdf:about="http://purl.obolibrary.org/obo/GAZ_22224105">
        <obo:RO_0001025 rdf:resource="http://purl.obolibrary.org/obo/GAZ_00002714"/>
        <oboInOwl:hasOBONamespace>GAZ</oboInOwl:hasOBONamespace>
        <oboInOwl:id>GAZ:22224105</oboInOwl:id>
        <rdfs:label>Hefer Valley Regional Council</rdfs:label>
    </owl:NamedIndividual>
    


    <!-- http://purl.obolibrary.org/obo/GAZ_22224107 -->

    <owl:NamedIndividual rdf:about="http://purl.obolibrary.org/obo/GAZ_22224107">
        <obo:RO_0001025 rdf:resource="http://purl.obolibrary.org/obo/GAZ_22224105"/>
        <oboInOwl:hasOBONamespace>GAZ</oboInOwl:hasOBONamespace>
        <oboInOwl:id>GAZ:22224107</oboInOwl:id>
        <rdfs:label>Moshavim Settlement</rdfs:label>
    </owl:NamedIndividual>
    


    <!-- http://purl.obolibrary.org/obo/GAZ_22224108 -->

    <owl:NamedIndividual rdf:about="http://purl.obolibrary.org/obo/GAZ_22224108">
        <obo:RO_0001025 rdf:resource="http://purl.obolibrary.org/obo/GAZ_22224107"/>
    </owl:NamedIndividual>
    


    <!-- 
    ///////////////////////////////////////////////////////////////////////////////////////
    //
    // Annotations
    //
    ///////////////////////////////////////////////////////////////////////////////////////
     -->

    <rdf:Description rdf:about="http://purl.obolibrary.org/obo/GAZ_00002705">
        <rdfs:label>populated place, Israel</rdfs:label>
        <oboInOwl:id>GAZ:00002705</oboInOwl:id>
        <oboInOwl:hasOBONamespace>GAZ</oboInOwl:hasOBONamespace>
    </rdf:Description>
    <rdf:Description rdf:about="http://purl.obolibrary.org/obo/GAZ_00002706">
        <obo:IAO_0000115>A populated place.</obo:IAO_0000115>
        <oboInOwl:hasOBONamespace>GAZ</oboInOwl:hasOBONamespace>
        <oboInOwl:id>GAZ:00002706</oboInOwl:id>
        <rdfs:label>Eilat</rdfs:label>
    </rdf:Description>
    <rdf:Description rdf:about="http://purl.obolibrary.org/obo/GAZ_00002707">
        <rdfs:label>District (Israel)</rdfs:label>
        <oboInOwl:hasOBONamespace>GAZ</oboInOwl:hasOBONamespace>
        <oboInOwl:id>GAZ:00002707</oboInOwl:id>
    </rdf:Description>
    <rdf:Description rdf:about="http://purl.obolibrary.org/obo/GAZ_00002708">
        <oboInOwl:hasOBONamespace>GAZ</oboInOwl:hasOBONamespace>
        <obo:IAO_0000115>One of six administrative districts of Israel.</obo:IAO_0000115>
        <oboInOwl:id>GAZ:00002708</oboInOwl:id>
        <rdfs:label>Jerusalem District</rdfs:label>
    </rdf:Description>
    <rdf:Description rdf:about="http://purl.obolibrary.org/obo/GAZ_00002709">
        <obo:IAO_0000115>One of six administrative districts of Israel.</obo:IAO_0000115>
        <oboInOwl:hasOBONamespace>GAZ</oboInOwl:hasOBONamespace>
        <oboInOwl:id>GAZ:00002709</oboInOwl:id>
        <rdfs:label>Tel Aviv District</rdfs:label>
    </rdf:Description>
    <rdf:Description rdf:about="http://purl.obolibrary.org/obo/GAZ_00002710">
        <oboInOwl:hasOBONamespace>GAZ</oboInOwl:hasOBONamespace>
        <obo:IAO_0000115>One of Israel&apos;s six administrative districts, and is the largest in terms of land area as well as the most sparsely populated. It covers most of the Negev desert, as well as the Arabah valley.</obo:IAO_0000115>
        <rdfs:label>Southern District</rdfs:label>
        <oboInOwl:id>GAZ:00002710</oboInOwl:id>
    </rdf:Description>
    <rdf:Description rdf:about="http://purl.obolibrary.org/obo/GAZ_00002711">
        <rdfs:label>Haifa District</rdfs:label>
        <oboInOwl:hasOBONamespace>GAZ</oboInOwl:hasOBONamespace>
        <obo:IAO_0000115>An administrative district surrounding the city of Haifa, Israel. The district is one of six administrative districts of Israel, and the capital of it is Haifa.</obo:IAO_0000115>
        <oboInOwl:id>GAZ:00002711</oboInOwl:id>
    </rdf:Description>
    <rdf:Description rdf:about="http://purl.obolibrary.org/obo/GAZ_00002712">
        <oboInOwl:id>GAZ:00002712</oboInOwl:id>
        <obo:IAO_0000115>One of the seven Districts of Israel (not recognised by the UN).</obo:IAO_0000115>
        <oboInOwl:hasOBONamespace>GAZ</oboInOwl:hasOBONamespace>
        <rdfs:label>Judea and Samaria Area (West Bank)</rdfs:label>
    </rdf:Description>
    <rdf:Description rdf:about="http://purl.obolibrary.org/obo/GAZ_00002713">
        <oboInOwl:id>GAZ:00002713</oboInOwl:id>
        <rdfs:label>Northern District</rdfs:label>
        <oboInOwl:hasOBONamespace>GAZ</oboInOwl:hasOBONamespace>
        <obo:IAO_0000115>One of Israels six administrative districts.</obo:IAO_0000115>
    </rdf:Description>
    <rdf:Description rdf:about="http://purl.obolibrary.org/obo/GAZ_00002714">
        <obo:IAO_0000115>One of six administrative districts, including most of the Sharon region. The district capital is Ramla.</obo:IAO_0000115>
        <oboInOwl:id>GAZ:00002714</oboInOwl:id>
        <oboInOwl:hasOBONamespace>GAZ</oboInOwl:hasOBONamespace>
        <rdfs:label>Center District</rdfs:label>
    </rdf:Description>
    <rdf:Description rdf:about="http://purl.obolibrary.org/obo/GAZ_00003782">
        <rdfs:label>Jerusalem</rdfs:label>
        <oboInOwl:id>GAZ:00003782</oboInOwl:id>
        <oboInOwl:hasOBONamespace>GAZ</oboInOwl:hasOBONamespace>
    </rdf:Description>
    <rdf:Description rdf:about="http://purl.obolibrary.org/obo/GAZ_00004382">
        <oboInOwl:id>GAZ:00004382</oboInOwl:id>
        <rdfs:label>Haifa</rdfs:label>
        <oboInOwl:hasOBONamespace>GAZ</oboInOwl:hasOBONamespace>
    </rdf:Description>
    <rdf:Description rdf:about="http://purl.obolibrary.org/obo/GAZ_00004383">
        <rdfs:label>Rehovot</rdfs:label>
        <obo:IAO_0000115>A populated place. A city in the Center District of Israel, about 20 km south of Tel Aviv.</obo:IAO_0000115>
        <oboInOwl:hasOBONamespace>GAZ</oboInOwl:hasOBONamespace>
        <oboInOwl:id>GAZ:00004383</oboInOwl:id>
    </rdf:Description>
    <rdf:Description rdf:about="http://purl.obolibrary.org/obo/GAZ_00008671">
        <obo:IAO_0000115>The second-largest city in Israel.</obo:IAO_0000115>
        <rdfs:label>Tel Aviv</rdfs:label>
        <oboInOwl:id>GAZ:00008671</oboInOwl:id>
        <oboInOwl:hasOBONamespace>GAZ</oboInOwl:hasOBONamespace>
    </rdf:Description>
    <rdf:Description rdf:about="http://purl.obolibrary.org/obo/GAZ_00010401">
        <rdfs:label>Amioz</rdfs:label>
        <oboInOwl:id>GAZ:00010401</oboInOwl:id>
        <oboInOwl:hasOBONamespace>GAZ</oboInOwl:hasOBONamespace>
    </rdf:Description>
    <rdf:Description rdf:about="http://purl.obolibrary.org/obo/GAZ_00010508">
        <oboInOwl:id>GAZ:00010508</oboInOwl:id>
        <oboInOwl:hasOBONamespace>GAZ</oboInOwl:hasOBONamespace>
        <rdfs:label>Avigdor</rdfs:label>
    </rdf:Description>
    <rdf:Description rdf:about="http://purl.obolibrary.org/obo/GAZ_00010510">
        <rdfs:label>Petah Tiqva</rdfs:label>
        <oboInOwl:hasOBONamespace>GAZ</oboInOwl:hasOBONamespace>
        <oboInOwl:id>GAZ:00010510</oboInOwl:id>
        <obo:IAO_0000115>A populated place. A city in the Center District of Israel, north-east of Tel Aviv.</obo:IAO_0000115>
    </rdf:Description>
    <rdf:Description rdf:about="http://purl.obolibrary.org/obo/GAZ_00010516">
        <oboInOwl:id>GAZ:00010516</oboInOwl:id>
        <rdfs:label>Ein Tzurim</rdfs:label>
        <obo:IAO_0000115>A religious kibbutz, located south of Kiryat Malakhi in south-central Israel. It is under the jurisdiction of Shafir Regional Council.</obo:IAO_0000115>
        <oboInOwl:hasOBONamespace>GAZ</oboInOwl:hasOBONamespace>
    </rdf:Description>
    <rdf:Description rdf:about="http://purl.obolibrary.org/obo/GAZ_00010520">
        <rdfs:label>Hadera</rdfs:label>
        <oboInOwl:id>GAZ:00010520</oboInOwl:id>
        <oboInOwl:hasOBONamespace>GAZ</oboInOwl:hasOBONamespace>
    </rdf:Description>
    <rdf:Description rdf:about="http://purl.obolibrary.org/obo/GAZ_00010525">
        <obo:IAO_0000115>An Israeli town in the Sharon region. It is located east of Netanya and north of Kfar Saba.</obo:IAO_0000115>
        <rdfs:label>Tel Mond</rdfs:label>
        <oboInOwl:id>GAZ:00010525</oboInOwl:id>
        <oboInOwl:hasOBONamespace>GAZ</oboInOwl:hasOBONamespace>
    </rdf:Description>
    <rdf:Description rdf:about="http://purl.obolibrary.org/obo/GAZ_00010528">
        <oboInOwl:id>GAZ:00010528</oboInOwl:id>
        <rdfs:label>Kfar Warburg</rdfs:label>
        <oboInOwl:hasOBONamespace>GAZ</oboInOwl:hasOBONamespace>
    </rdf:Description>
    <rdf:Description rdf:about="http://purl.obolibrary.org/obo/GAZ_00010529">
        <oboInOwl:id>GAZ:00010529</oboInOwl:id>
        <rdfs:label>Ma&apos;anit</rdfs:label>
        <oboInOwl:hasOBONamespace>GAZ</oboInOwl:hasOBONamespace>
        <obo:IAO_0000115>A kibbutz located near the town of Pardes Hanna-Karkur in northern Israel. It falls under the jurisdiction of Menashe Regional Council.</obo:IAO_0000115>
    </rdf:Description>
    <rdf:Description rdf:about="http://purl.obolibrary.org/obo/GAZ_00010530">
        <obo:IAO_0000115>A settlement in the Jezreel Valley Regional Council.</obo:IAO_0000115>
        <oboInOwl:id>GAZ:00010530</oboInOwl:id>
        <oboInOwl:hasOBONamespace>GAZ</oboInOwl:hasOBONamespace>
        <rdfs:label>Tel Adashim</rdfs:label>
    </rdf:Description>
    <rdf:Description rdf:about="http://purl.obolibrary.org/obo/GAZ_00010531">
        <rdfs:label>Nahalal</rdfs:label>
        <oboInOwl:id>GAZ:00010531</oboInOwl:id>
        <oboInOwl:hasOBONamespace>GAZ</oboInOwl:hasOBONamespace>
        <obo:IAO_0000115>A moshav in Israel&apos;s Jezreel Valley.</obo:IAO_0000115>
    </rdf:Description>
    <rdf:Description rdf:about="http://purl.obolibrary.org/obo/GAZ_00010536">
        <rdfs:label>City of Nahariya</rdfs:label>
        <oboInOwl:hasOBONamespace>GAZ</oboInOwl:hasOBONamespace>
        <obo:IAO_0000115>A city located in the North District of Israel on the Mediterranean sea, just south of the Lebanese border at Rosh HaNikra.</obo:IAO_0000115>
        <oboInOwl:id>GAZ:00010536</oboInOwl:id>
    </rdf:Description>
    <rdf:Description rdf:about="http://purl.obolibrary.org/obo/GAZ_00010537">
        <rdfs:label>Sde Uziyahu</rdfs:label>
        <oboInOwl:id>GAZ:00010537</oboInOwl:id>
        <oboInOwl:hasOBONamespace>GAZ</oboInOwl:hasOBONamespace>
    </rdf:Description>
    <rdf:Description rdf:about="http://purl.obolibrary.org/obo/GAZ_00010541">
        <oboInOwl:id>GAZ:00010541</oboInOwl:id>
        <rdfs:label>Talmei Elazar</rdfs:label>
        <obo:IAO_0000115>A moshav in the Menashe Regional Council.</obo:IAO_0000115>
        <oboInOwl:hasOBONamespace>GAZ</oboInOwl:hasOBONamespace>
    </rdf:Description>
    <rdf:Description rdf:about="http://purl.obolibrary.org/obo/GAZ_22224108">
        <oboInOwl:id>GAZ:22224108</oboInOwl:id>
        <oboInOwl:hasOBONamespace>GAZ</oboInOwl:hasOBONamespace>
        <rdfs:label>Beit Herut</rdfs:label>
    </rdf:Description>
</rdf:RDF>



<!-- Generated by the OWL API (version 4.5.6) https://github.com/owlcs/owlapi -->

