<?xml version="1.0"?>
<rdf:RDF xmlns="http://purl.obolibrary.org/obo/gaz/subsets/countries/Jamaica.owl#"
     xml:base="http://purl.obolibrary.org/obo/gaz/subsets/countries/Jamaica.owl"
     xmlns:obo="http://purl.obolibrary.org/obo/"
     xmlns:owl="http://www.w3.org/2002/07/owl#"
     xmlns:rdf="http://www.w3.org/1999/02/22-rdf-syntax-ns#"
     xmlns:xml="http://www.w3.org/XML/1998/namespace"
     xmlns:xsd="http://www.w3.org/2001/XMLSchema#"
     xmlns:rdfs="http://www.w3.org/2000/01/rdf-schema#"
     xmlns:oboInOwl="http://www.geneontology.org/formats/oboInOwl#">
    <owl:Ontology rdf:about="http://purl.obolibrary.org/obo/gaz/subsets/countries/Jamaica.owl">
        <owl:imports rdf:resource="http://purl.obolibrary.org/obo/gaz/imports/envo_import.owl"/>
        <owl:imports rdf:resource="http://purl.obolibrary.org/obo/gaz/imports/ro_import.owl"/>
    </owl:Ontology>
    


    <!-- 
    ///////////////////////////////////////////////////////////////////////////////////////
    //
    // Annotation properties
    //
    ///////////////////////////////////////////////////////////////////////////////////////
     -->

    


    <!-- http://purl.obolibrary.org/obo/IAO_0000115 -->

    <owl:AnnotationProperty rdf:about="http://purl.obolibrary.org/obo/IAO_0000115"/>
    


    <!-- http://www.geneontology.org/formats/oboInOwl#hasOBONamespace -->

    <owl:AnnotationProperty rdf:about="http://www.geneontology.org/formats/oboInOwl#hasOBONamespace"/>
    


    <!-- http://www.geneontology.org/formats/oboInOwl#id -->

    <owl:AnnotationProperty rdf:about="http://www.geneontology.org/formats/oboInOwl#id"/>
    


    <!-- 
    ///////////////////////////////////////////////////////////////////////////////////////
    //
    // Object Properties
    //
    ///////////////////////////////////////////////////////////////////////////////////////
     -->

    


    <!-- http://purl.obolibrary.org/obo/RO_0001025 -->

    <owl:ObjectProperty rdf:about="http://purl.obolibrary.org/obo/RO_0001025"/>
    


    <!-- 
    ///////////////////////////////////////////////////////////////////////////////////////
    //
    // Classes
    //
    ///////////////////////////////////////////////////////////////////////////////////////
     -->

    


    <!-- http://purl.obolibrary.org/obo/ENVO_00000106 -->

    <owl:Class rdf:about="http://purl.obolibrary.org/obo/ENVO_00000106"/>
    


    <!-- http://purl.obolibrary.org/obo/ENVO_00000167 -->

    <owl:Class rdf:about="http://purl.obolibrary.org/obo/ENVO_00000167"/>
    


    <!-- http://purl.obolibrary.org/obo/ENVO_00000175 -->

    <owl:Class rdf:about="http://purl.obolibrary.org/obo/ENVO_00000175"/>
    


    <!-- http://purl.obolibrary.org/obo/ENVO_00000856 -->

    <owl:Class rdf:about="http://purl.obolibrary.org/obo/ENVO_00000856"/>
    


    <!-- http://purl.obolibrary.org/obo/GAZ_00004312 -->

    <owl:Class rdf:about="http://purl.obolibrary.org/obo/GAZ_00004312"/>
    


    <!-- http://purl.obolibrary.org/obo/GAZ_00008621 -->

    <owl:Class rdf:about="http://purl.obolibrary.org/obo/GAZ_00008621">
        <rdfs:subClassOf rdf:resource="http://purl.obolibrary.org/obo/GAZ_00008622"/>
        <oboInOwl:hasOBONamespace>GAZ</oboInOwl:hasOBONamespace>
        <oboInOwl:id>GAZ:00008621</oboInOwl:id>
        <rdfs:label>Montego Bay</rdfs:label>
    </owl:Class>
    


    <!-- http://purl.obolibrary.org/obo/GAZ_00008622 -->

    <owl:Class rdf:about="http://purl.obolibrary.org/obo/GAZ_00008622"/>
    


    <!-- http://purl.obolibrary.org/obo/GAZ_00010072 -->

    <owl:Class rdf:about="http://purl.obolibrary.org/obo/GAZ_00010072">
        <rdfs:subClassOf rdf:resource="http://purl.obolibrary.org/obo/GAZ_00008622"/>
    </owl:Class>
    


    <!-- http://purl.obolibrary.org/obo/GAZ_00013516 -->

    <owl:Class rdf:about="http://purl.obolibrary.org/obo/GAZ_00013516">
        <rdfs:subClassOf rdf:resource="http://purl.obolibrary.org/obo/GAZ_00004312"/>
    </owl:Class>
    


    <!-- http://purl.obolibrary.org/obo/GAZ_00013517 -->

    <owl:Class rdf:about="http://purl.obolibrary.org/obo/GAZ_00013517">
        <rdfs:subClassOf rdf:resource="http://purl.obolibrary.org/obo/GAZ_00004312"/>
    </owl:Class>
    


    <!-- http://purl.obolibrary.org/obo/GAZ_00013518 -->

    <owl:Class rdf:about="http://purl.obolibrary.org/obo/GAZ_00013518">
        <rdfs:subClassOf rdf:resource="http://purl.obolibrary.org/obo/GAZ_00004312"/>
    </owl:Class>
    


    <!-- 
    ///////////////////////////////////////////////////////////////////////////////////////
    //
    // Individuals
    //
    ///////////////////////////////////////////////////////////////////////////////////////
     -->

    


    <!-- http://purl.obolibrary.org/obo/GAZ_00003781 -->

    <owl:NamedIndividual rdf:about="http://purl.obolibrary.org/obo/GAZ_00003781">
        <obo:IAO_0000115>A nation of the Greater Antilles. Jamaica is divided into 14 parishes, which are grouped into three historic counties that have no administrative relevance.</obo:IAO_0000115>
        <oboInOwl:hasOBONamespace>GAZ</oboInOwl:hasOBONamespace>
        <oboInOwl:id>GAZ:00003781</oboInOwl:id>
        <rdfs:label>Jamaica</rdfs:label>
    </owl:NamedIndividual>
    


    <!-- http://purl.obolibrary.org/obo/GAZ_00004312 -->

    <owl:NamedIndividual rdf:about="http://purl.obolibrary.org/obo/GAZ_00004312">
        <obo:RO_0001025 rdf:resource="http://purl.obolibrary.org/obo/GAZ_00003781"/>
    </owl:NamedIndividual>
    


    <!-- http://purl.obolibrary.org/obo/GAZ_00004339 -->

    <owl:NamedIndividual rdf:about="http://purl.obolibrary.org/obo/GAZ_00004339">
        <obo:RO_0001025 rdf:resource="http://purl.obolibrary.org/obo/GAZ_00013517"/>
        <obo:IAO_0000115>A parish located on Jamaica&apos;s northeast coast. It is situated to the north of St. Thomas, and the east of St. Mary in Surrey county.</obo:IAO_0000115>
        <oboInOwl:hasOBONamespace>GAZ</oboInOwl:hasOBONamespace>
        <oboInOwl:id>GAZ:00004339</oboInOwl:id>
        <rdfs:label>Portland Parish</rdfs:label>
    </owl:NamedIndividual>
    


    <!-- http://purl.obolibrary.org/obo/GAZ_00008620 -->

    <owl:NamedIndividual rdf:about="http://purl.obolibrary.org/obo/GAZ_00008620">
        <rdf:type rdf:resource="http://purl.obolibrary.org/obo/ENVO_00000856"/>
        <obo:RO_0001025 rdf:resource="http://purl.obolibrary.org/obo/GAZ_00013508"/>
        <obo:IAO_0000115>A populated place. A small town in Saint Ann, Jamaica.</obo:IAO_0000115>
        <oboInOwl:hasOBONamespace>GAZ</oboInOwl:hasOBONamespace>
        <oboInOwl:id>GAZ:00008620</oboInOwl:id>
        <rdfs:label>Moneague</rdfs:label>
    </owl:NamedIndividual>
    


    <!-- http://purl.obolibrary.org/obo/GAZ_00008622 -->

    <owl:NamedIndividual rdf:about="http://purl.obolibrary.org/obo/GAZ_00008622">
        <obo:RO_0001025 rdf:resource="http://purl.obolibrary.org/obo/GAZ_00003781"/>
    </owl:NamedIndividual>
    


    <!-- http://purl.obolibrary.org/obo/GAZ_00010070 -->

    <owl:NamedIndividual rdf:about="http://purl.obolibrary.org/obo/GAZ_00010070">
        <obo:RO_0001025 rdf:resource="http://purl.obolibrary.org/obo/GAZ_00013516"/>
        <obo:IAO_0000115>A parish, located on the northwestern tip of the island of Jamaica. It is a part of the county of Cornwall, bordered by St. James in the east, and Westmoreland in the south. With the exception of Kingston.</obo:IAO_0000115>
        <oboInOwl:hasOBONamespace>GAZ</oboInOwl:hasOBONamespace>
        <oboInOwl:id>GAZ:00010070</oboInOwl:id>
        <rdfs:label>Hanover Parish</rdfs:label>
    </owl:NamedIndividual>
    


    <!-- http://purl.obolibrary.org/obo/GAZ_00010071 -->

    <owl:NamedIndividual rdf:about="http://purl.obolibrary.org/obo/GAZ_00010071">
        <obo:RO_0001025 rdf:resource="http://purl.obolibrary.org/obo/GAZ_00013516"/>
        <obo:IAO_0000115>The westernmost parish in Jamaica, located on the south side of the island. It is situated to the south of Hanover, the southwest of Saint James, and the northwest of Saint Elizabeth, in the county of Cornwall. The chief town and capital is Savanna-la-Mar.</obo:IAO_0000115>
        <oboInOwl:hasOBONamespace>GAZ</oboInOwl:hasOBONamespace>
        <oboInOwl:id>GAZ:00010071</oboInOwl:id>
        <rdfs:label>Westmoreland Parish</rdfs:label>
    </owl:NamedIndividual>
    


    <!-- http://purl.obolibrary.org/obo/GAZ_00010072 -->

    <owl:NamedIndividual rdf:about="http://purl.obolibrary.org/obo/GAZ_00010072">
        <obo:RO_0001025 rdf:resource="http://purl.obolibrary.org/obo/GAZ_00010070"/>
        <obo:RO_0001025 rdf:resource="http://purl.obolibrary.org/obo/GAZ_00010071"/>
    </owl:NamedIndividual>
    


    <!-- http://purl.obolibrary.org/obo/GAZ_00013505 -->

    <owl:NamedIndividual rdf:about="http://purl.obolibrary.org/obo/GAZ_00013505">
        <obo:RO_0001025 rdf:resource="http://purl.obolibrary.org/obo/GAZ_00013517"/>
        <obo:IAO_0000115>A parish, situated in the southeast of Jamaica in the county of Surrey. It lies north of Kingston, stretches into the Blue Mountains. The parish lies just north of Kingston, bounded in the west by St. Catherine, north by St. Mary, northeast by Portland along the Blue Mountain range, and east by St. Thomas.</obo:IAO_0000115>
        <oboInOwl:hasOBONamespace>GAZ</oboInOwl:hasOBONamespace>
        <oboInOwl:id>GAZ:00013505</oboInOwl:id>
        <rdfs:label>Saint Andrew Parish</rdfs:label>
    </owl:NamedIndividual>
    


    <!-- http://purl.obolibrary.org/obo/GAZ_00013506 -->

    <owl:NamedIndividual rdf:about="http://purl.obolibrary.org/obo/GAZ_00013506">
        <obo:RO_0001025 rdf:resource="http://purl.obolibrary.org/obo/GAZ_00013517"/>
        <obo:IAO_0000115>A parish of Jamaica. It does not include the whole city of Kingston, it only consists of old downtown Kingston and Port Royal.</obo:IAO_0000115>
        <oboInOwl:hasOBONamespace>GAZ</oboInOwl:hasOBONamespace>
        <oboInOwl:id>GAZ:00013506</oboInOwl:id>
        <rdfs:label>Kingston Parish</rdfs:label>
    </owl:NamedIndividual>
    


    <!-- http://purl.obolibrary.org/obo/GAZ_00013507 -->

    <owl:NamedIndividual rdf:about="http://purl.obolibrary.org/obo/GAZ_00013507">
        <obo:RO_0001025 rdf:resource="http://purl.obolibrary.org/obo/GAZ_00013518"/>
        <obo:IAO_0000115>A Parish located in west-central Jamaica, in the county of Middlesex. Its capital, Mandeville. It is bordered by St. Elizabeth in the west, Clarendon in the east and by Trelawny in the north.</obo:IAO_0000115>
        <oboInOwl:hasOBONamespace>GAZ</oboInOwl:hasOBONamespace>
        <oboInOwl:id>GAZ:00013507</oboInOwl:id>
        <rdfs:label>Manchester Parish</rdfs:label>
    </owl:NamedIndividual>
    


    <!-- http://purl.obolibrary.org/obo/GAZ_00013508 -->

    <owl:NamedIndividual rdf:about="http://purl.obolibrary.org/obo/GAZ_00013508">
        <obo:RO_0001025 rdf:resource="http://purl.obolibrary.org/obo/GAZ_00013518"/>
        <obo:IAO_0000115>The largest parish in Jamaica. It is situated on the north coast of the island, in the county of Middlesex, roughly halfway between the eastern and western ends of the island. It is bordered on the south by Clarendon and St. Catherine, in the east by Saint Mary, and Trelawny in the west.</obo:IAO_0000115>
        <oboInOwl:hasOBONamespace>GAZ</oboInOwl:hasOBONamespace>
        <oboInOwl:id>GAZ:00013508</oboInOwl:id>
        <rdfs:label>Saint Ann Parish</rdfs:label>
    </owl:NamedIndividual>
    


    <!-- http://purl.obolibrary.org/obo/GAZ_00013509 -->

    <owl:NamedIndividual rdf:about="http://purl.obolibrary.org/obo/GAZ_00013509">
        <obo:RO_0001025 rdf:resource="http://purl.obolibrary.org/obo/GAZ_00013518"/>
        <obo:IAO_0000115>A parish in Jamaica. It is located on the south of the island, roughly half-way between the island&apos;s eastern and western ends. Located in the county of Middlesex, it is bordered by Manchester on the west, Saint Catherine in the east, and in the north by Saint Ann.</obo:IAO_0000115>
        <oboInOwl:hasOBONamespace>GAZ</oboInOwl:hasOBONamespace>
        <oboInOwl:id>GAZ:00013509</oboInOwl:id>
        <rdfs:label>Clarendon Parish</rdfs:label>
    </owl:NamedIndividual>
    


    <!-- http://purl.obolibrary.org/obo/GAZ_00013510 -->

    <owl:NamedIndividual rdf:about="http://purl.obolibrary.org/obo/GAZ_00013510">
        <obo:RO_0001025 rdf:resource="http://purl.obolibrary.org/obo/GAZ_00013516"/>
        <obo:IAO_0000115>A parish, located on the north west end of the island of Jamaica. The parish is bordered by Trelawny in the east, St. Elizabeth in the south and Hanover and Westmoreland in the west.</obo:IAO_0000115>
        <oboInOwl:hasOBONamespace>GAZ</oboInOwl:hasOBONamespace>
        <oboInOwl:id>GAZ:00013510</oboInOwl:id>
        <rdfs:label>Saint James Parish</rdfs:label>
    </owl:NamedIndividual>
    


    <!-- http://purl.obolibrary.org/obo/GAZ_00013511 -->

    <owl:NamedIndividual rdf:about="http://purl.obolibrary.org/obo/GAZ_00013511">
        <obo:RO_0001025 rdf:resource="http://purl.obolibrary.org/obo/GAZ_00013516"/>
        <obo:IAO_0000115>A parish in the County of Cornwall, Jamaica, located in the southwest of the island, in the county of Cornwall. It is to the west of Manchester, the east of Westmoreland, and to the south of St. James and Trelawny.</obo:IAO_0000115>
        <oboInOwl:hasOBONamespace>GAZ</oboInOwl:hasOBONamespace>
        <oboInOwl:id>GAZ:00013511</oboInOwl:id>
        <rdfs:label>Saint Elizabeth Parish</rdfs:label>
    </owl:NamedIndividual>
    


    <!-- http://purl.obolibrary.org/obo/GAZ_00013512 -->

    <owl:NamedIndividual rdf:about="http://purl.obolibrary.org/obo/GAZ_00013512">
        <obo:RO_0001025 rdf:resource="http://purl.obolibrary.org/obo/GAZ_00013518"/>
        <obo:IAO_0000115>A parish located in the south east of Jamaica. It is located in the county of Middlesex. It is bordered by St Andrew in the east, Clarendon in the west, and by St Mary and St Ann in the north.</obo:IAO_0000115>
        <oboInOwl:hasOBONamespace>GAZ</oboInOwl:hasOBONamespace>
        <oboInOwl:id>GAZ:00013512</oboInOwl:id>
        <rdfs:label>Saint Catherine Parish</rdfs:label>
    </owl:NamedIndividual>
    


    <!-- http://purl.obolibrary.org/obo/GAZ_00013513 -->

    <owl:NamedIndividual rdf:about="http://purl.obolibrary.org/obo/GAZ_00013513">
        <obo:RO_0001025 rdf:resource="http://purl.obolibrary.org/obo/GAZ_00013517"/>
        <obo:IAO_0000115>A parish that is situated at the south eastern end of Jamaica, in the county of Surrey. It is located to the south of Portland, and the east of St. Andrew.</obo:IAO_0000115>
        <oboInOwl:hasOBONamespace>GAZ</oboInOwl:hasOBONamespace>
        <oboInOwl:id>GAZ:00013513</oboInOwl:id>
        <rdfs:label>Saint Thomas Parish</rdfs:label>
    </owl:NamedIndividual>
    


    <!-- http://purl.obolibrary.org/obo/GAZ_00013514 -->

    <owl:NamedIndividual rdf:about="http://purl.obolibrary.org/obo/GAZ_00013514">
        <obo:RO_0001025 rdf:resource="http://purl.obolibrary.org/obo/GAZ_00013516"/>
        <obo:IAO_0000115>A parish located on the northwest section of Jamaica in the county of Cornwall. Its capital is Falmouth. It is bordered by Saint Ann in the east, Saint James in the west, and parts of Saint Elizabeth and Manchester in the south.</obo:IAO_0000115>
        <oboInOwl:hasOBONamespace>GAZ</oboInOwl:hasOBONamespace>
        <oboInOwl:id>GAZ:00013514</oboInOwl:id>
        <rdfs:label>Trelawny Parish</rdfs:label>
    </owl:NamedIndividual>
    


    <!-- http://purl.obolibrary.org/obo/GAZ_00013515 -->

    <owl:NamedIndividual rdf:about="http://purl.obolibrary.org/obo/GAZ_00013515">
        <obo:RO_0001025 rdf:resource="http://purl.obolibrary.org/obo/GAZ_00013518"/>
        <obo:IAO_0000115>A parish located in the northeast section of Jamaica. It is one of Jamaica&apos;s smallest parishes, located in the county of Middlesex. Its chief town and capital is Port Maria, located on the coast. It is bordered by Portland in the east, St. Ann in the west, and parts of St. Catherine and St. Andrew in the south.</obo:IAO_0000115>
        <oboInOwl:hasOBONamespace>GAZ</oboInOwl:hasOBONamespace>
        <oboInOwl:id>GAZ:00013515</oboInOwl:id>
        <rdfs:label>Saint Mary Parish</rdfs:label>
    </owl:NamedIndividual>
    


    <!-- http://purl.obolibrary.org/obo/GAZ_00013516 -->

    <owl:NamedIndividual rdf:about="http://purl.obolibrary.org/obo/GAZ_00013516"/>
    


    <!-- http://purl.obolibrary.org/obo/GAZ_00013517 -->

    <owl:NamedIndividual rdf:about="http://purl.obolibrary.org/obo/GAZ_00013517"/>
    


    <!-- http://purl.obolibrary.org/obo/GAZ_00013518 -->

    <owl:NamedIndividual rdf:about="http://purl.obolibrary.org/obo/GAZ_00013518"/>
    


    <!-- http://purl.obolibrary.org/obo/GAZ_00049733 -->

    <owl:NamedIndividual rdf:about="http://purl.obolibrary.org/obo/GAZ_00049733">
        <obo:RO_0001025 rdf:resource="http://purl.obolibrary.org/obo/GAZ_00013509"/>
        <obo:RO_0001025 rdf:resource="http://purl.obolibrary.org/obo/GAZ_00251113"/>
        <obo:IAO_0000115>An island.</obo:IAO_0000115>
        <oboInOwl:hasOBONamespace>GAZ</oboInOwl:hasOBONamespace>
        <oboInOwl:id>GAZ:00049733</oboInOwl:id>
        <rdfs:label>Dolphin Island</rdfs:label>
    </owl:NamedIndividual>
    


    <!-- http://purl.obolibrary.org/obo/GAZ_00049734 -->

    <owl:NamedIndividual rdf:about="http://purl.obolibrary.org/obo/GAZ_00049734">
        <obo:RO_0001025 rdf:resource="http://purl.obolibrary.org/obo/GAZ_00013512"/>
        <obo:RO_0001025 rdf:resource="http://purl.obolibrary.org/obo/GAZ_00251113"/>
        <obo:IAO_0000115>An island.</obo:IAO_0000115>
        <oboInOwl:hasOBONamespace>GAZ</oboInOwl:hasOBONamespace>
        <oboInOwl:id>GAZ:00049734</oboInOwl:id>
        <rdfs:label>Little Goat Island</rdfs:label>
    </owl:NamedIndividual>
    


    <!-- http://purl.obolibrary.org/obo/GAZ_00049735 -->

    <owl:NamedIndividual rdf:about="http://purl.obolibrary.org/obo/GAZ_00049735">
        <obo:RO_0001025 rdf:resource="http://purl.obolibrary.org/obo/GAZ_00013512"/>
        <obo:RO_0001025 rdf:resource="http://purl.obolibrary.org/obo/GAZ_00251113"/>
        <obo:IAO_0000115>An island.</obo:IAO_0000115>
        <oboInOwl:hasOBONamespace>GAZ</oboInOwl:hasOBONamespace>
        <oboInOwl:id>GAZ:00049735</oboInOwl:id>
        <rdfs:label>Great Goat Island</rdfs:label>
    </owl:NamedIndividual>
    


    <!-- http://purl.obolibrary.org/obo/GAZ_00049736 -->

    <owl:NamedIndividual rdf:about="http://purl.obolibrary.org/obo/GAZ_00049736">
        <obo:RO_0001025 rdf:resource="http://purl.obolibrary.org/obo/GAZ_00251085"/>
        <obo:IAO_0000115>Islands.</obo:IAO_0000115>
        <oboInOwl:hasOBONamespace>GAZ</oboInOwl:hasOBONamespace>
        <oboInOwl:id>GAZ:00049736</oboInOwl:id>
        <rdfs:label>Bogue Islands</rdfs:label>
    </owl:NamedIndividual>
    


    <!-- http://purl.obolibrary.org/obo/GAZ_00049737 -->

    <owl:NamedIndividual rdf:about="http://purl.obolibrary.org/obo/GAZ_00049737">
        <obo:RO_0001025 rdf:resource="http://purl.obolibrary.org/obo/GAZ_00010070"/>
        <obo:IAO_0000115>An island.</obo:IAO_0000115>
        <oboInOwl:hasOBONamespace>GAZ</oboInOwl:hasOBONamespace>
        <oboInOwl:id>GAZ:00049737</oboInOwl:id>
        <rdfs:label>Booby Cay</rdfs:label>
    </owl:NamedIndividual>
    


    <!-- http://purl.obolibrary.org/obo/GAZ_00049738 -->

    <owl:NamedIndividual rdf:about="http://purl.obolibrary.org/obo/GAZ_00049738">
        <obo:RO_0001025 rdf:resource="http://purl.obolibrary.org/obo/GAZ_00013509"/>
        <obo:RO_0001025 rdf:resource="http://purl.obolibrary.org/obo/GAZ_00251113"/>
        <obo:IAO_0000115>An island.</obo:IAO_0000115>
        <oboInOwl:hasOBONamespace>GAZ</oboInOwl:hasOBONamespace>
        <oboInOwl:id>GAZ:00049738</oboInOwl:id>
        <rdfs:label>Big Half Moon Cay</rdfs:label>
    </owl:NamedIndividual>
    


    <!-- http://purl.obolibrary.org/obo/GAZ_00049739 -->

    <owl:NamedIndividual rdf:about="http://purl.obolibrary.org/obo/GAZ_00049739">
        <obo:RO_0001025 rdf:resource="http://purl.obolibrary.org/obo/GAZ_00003781"/>
        <obo:IAO_0000115>An island.</obo:IAO_0000115>
        <oboInOwl:hasOBONamespace>GAZ</oboInOwl:hasOBONamespace>
        <oboInOwl:id>GAZ:00049739</oboInOwl:id>
        <rdfs:label>Bumpduklok</rdfs:label>
    </owl:NamedIndividual>
    


    <!-- http://purl.obolibrary.org/obo/GAZ_00049740 -->

    <owl:NamedIndividual rdf:about="http://purl.obolibrary.org/obo/GAZ_00049740">
        <obo:RO_0001025 rdf:resource="http://purl.obolibrary.org/obo/GAZ_00013513"/>
        <obo:IAO_0000115>An island.</obo:IAO_0000115>
        <oboInOwl:hasOBONamespace>GAZ</oboInOwl:hasOBONamespace>
        <oboInOwl:id>GAZ:00049740</oboInOwl:id>
        <rdfs:label>Emerald Island</rdfs:label>
    </owl:NamedIndividual>
    


    <!-- http://purl.obolibrary.org/obo/GAZ_00049741 -->

    <owl:NamedIndividual rdf:about="http://purl.obolibrary.org/obo/GAZ_00049741">
        <obo:RO_0001025 rdf:resource="http://purl.obolibrary.org/obo/GAZ_00003781"/>
        <obo:IAO_0000115>A small group of uninhabited islands or cays off Port Royal, Jamaica.</obo:IAO_0000115>
        <oboInOwl:hasOBONamespace>GAZ</oboInOwl:hasOBONamespace>
        <oboInOwl:id>GAZ:00049741</oboInOwl:id>
        <rdfs:label>Port Royal Cays</rdfs:label>
    </owl:NamedIndividual>
    


    <!-- http://purl.obolibrary.org/obo/GAZ_00049742 -->

    <owl:NamedIndividual rdf:about="http://purl.obolibrary.org/obo/GAZ_00049742">
        <obo:RO_0001025 rdf:resource="http://purl.obolibrary.org/obo/GAZ_00049741"/>
        <obo:IAO_0000115>One of the Port Royal Cays.</obo:IAO_0000115>
        <oboInOwl:hasOBONamespace>GAZ</oboInOwl:hasOBONamespace>
        <oboInOwl:id>GAZ:00049742</oboInOwl:id>
        <rdfs:label>Lime Cay</rdfs:label>
    </owl:NamedIndividual>
    


    <!-- http://purl.obolibrary.org/obo/GAZ_00049743 -->

    <owl:NamedIndividual rdf:about="http://purl.obolibrary.org/obo/GAZ_00049743">
        <obo:RO_0001025 rdf:resource="http://purl.obolibrary.org/obo/GAZ_00049741"/>
        <obo:IAO_0000115>One of the Port Royal Cays.</obo:IAO_0000115>
        <oboInOwl:hasOBONamespace>GAZ</oboInOwl:hasOBONamespace>
        <oboInOwl:id>GAZ:00049743</oboInOwl:id>
        <rdfs:label>Gun Cay</rdfs:label>
    </owl:NamedIndividual>
    


    <!-- http://purl.obolibrary.org/obo/GAZ_00049744 -->

    <owl:NamedIndividual rdf:about="http://purl.obolibrary.org/obo/GAZ_00049744">
        <obo:RO_0001025 rdf:resource="http://purl.obolibrary.org/obo/GAZ_00049741"/>
        <obo:IAO_0000115>One of the Port Royal Cays.</obo:IAO_0000115>
        <oboInOwl:hasOBONamespace>GAZ</oboInOwl:hasOBONamespace>
        <oboInOwl:id>GAZ:00049744</oboInOwl:id>
        <rdfs:label>Maiden Cay</rdfs:label>
    </owl:NamedIndividual>
    


    <!-- http://purl.obolibrary.org/obo/GAZ_00049745 -->

    <owl:NamedIndividual rdf:about="http://purl.obolibrary.org/obo/GAZ_00049745">
        <obo:RO_0001025 rdf:resource="http://purl.obolibrary.org/obo/GAZ_00049741"/>
        <obo:IAO_0000115>One of the Port Royal Cays.</obo:IAO_0000115>
        <oboInOwl:hasOBONamespace>GAZ</oboInOwl:hasOBONamespace>
        <oboInOwl:id>GAZ:00049745</oboInOwl:id>
        <rdfs:label>Southeast Cay</rdfs:label>
    </owl:NamedIndividual>
    


    <!-- http://purl.obolibrary.org/obo/GAZ_00049746 -->

    <owl:NamedIndividual rdf:about="http://purl.obolibrary.org/obo/GAZ_00049746">
        <obo:RO_0001025 rdf:resource="http://purl.obolibrary.org/obo/GAZ_00049741"/>
        <obo:IAO_0000115>One of the Port Royal Cays.</obo:IAO_0000115>
        <oboInOwl:hasOBONamespace>GAZ</oboInOwl:hasOBONamespace>
        <oboInOwl:id>GAZ:00049746</oboInOwl:id>
        <rdfs:label>Drunkenmans Cay</rdfs:label>
    </owl:NamedIndividual>
    


    <!-- http://purl.obolibrary.org/obo/GAZ_00049747 -->

    <owl:NamedIndividual rdf:about="http://purl.obolibrary.org/obo/GAZ_00049747">
        <obo:RO_0001025 rdf:resource="http://purl.obolibrary.org/obo/GAZ_00049741"/>
        <obo:IAO_0000115>One of the Port Royal Cays.</obo:IAO_0000115>
        <oboInOwl:hasOBONamespace>GAZ</oboInOwl:hasOBONamespace>
        <oboInOwl:id>GAZ:00049747</oboInOwl:id>
        <rdfs:label>Rackhams Cay</rdfs:label>
    </owl:NamedIndividual>
    


    <!-- http://purl.obolibrary.org/obo/GAZ_00049748 -->

    <owl:NamedIndividual rdf:about="http://purl.obolibrary.org/obo/GAZ_00049748">
        <obo:RO_0001025 rdf:resource="http://purl.obolibrary.org/obo/GAZ_00049741"/>
        <obo:IAO_0000115>One of the Port Royal Cays.</obo:IAO_0000115>
        <oboInOwl:hasOBONamespace>GAZ</oboInOwl:hasOBONamespace>
        <oboInOwl:id>GAZ:00049748</oboInOwl:id>
        <rdfs:label>South Cay</rdfs:label>
    </owl:NamedIndividual>
    


    <!-- http://purl.obolibrary.org/obo/GAZ_00049749 -->

    <owl:NamedIndividual rdf:about="http://purl.obolibrary.org/obo/GAZ_00049749">
        <obo:RO_0001025 rdf:resource="http://purl.obolibrary.org/obo/GAZ_00049741"/>
        <obo:IAO_0000115>One of the Port Royal Cays.</obo:IAO_0000115>
        <oboInOwl:hasOBONamespace>GAZ</oboInOwl:hasOBONamespace>
        <oboInOwl:id>GAZ:00049749</oboInOwl:id>
        <rdfs:label>South Cay Rock</rdfs:label>
    </owl:NamedIndividual>
    


    <!-- http://purl.obolibrary.org/obo/GAZ_00049750 -->

    <owl:NamedIndividual rdf:about="http://purl.obolibrary.org/obo/GAZ_00049750">
        <obo:RO_0001025 rdf:resource="http://purl.obolibrary.org/obo/GAZ_00251085"/>
        <obo:IAO_0000115>An island.</obo:IAO_0000115>
        <oboInOwl:hasOBONamespace>GAZ</oboInOwl:hasOBONamespace>
        <oboInOwl:id>GAZ:00049750</oboInOwl:id>
        <rdfs:label>Kokomo Island</rdfs:label>
    </owl:NamedIndividual>
    


    <!-- http://purl.obolibrary.org/obo/GAZ_00049751 -->

    <owl:NamedIndividual rdf:about="http://purl.obolibrary.org/obo/GAZ_00049751">
        <obo:RO_0001025 rdf:resource="http://purl.obolibrary.org/obo/GAZ_00013509"/>
        <obo:RO_0001025 rdf:resource="http://purl.obolibrary.org/obo/GAZ_00251113"/>
        <obo:IAO_0000115>An island.</obo:IAO_0000115>
        <oboInOwl:hasOBONamespace>GAZ</oboInOwl:hasOBONamespace>
        <oboInOwl:id>GAZ:00049751</oboInOwl:id>
        <rdfs:label>Little Half Moon Cay</rdfs:label>
    </owl:NamedIndividual>
    


    <!-- http://purl.obolibrary.org/obo/GAZ_00049752 -->

    <owl:NamedIndividual rdf:about="http://purl.obolibrary.org/obo/GAZ_00049752">
        <obo:RO_0001025 rdf:resource="http://purl.obolibrary.org/obo/GAZ_00003781"/>
        <oboInOwl:hasOBONamespace>GAZ</oboInOwl:hasOBONamespace>
        <oboInOwl:id>GAZ:00049752</oboInOwl:id>
        <rdfs:label>Morant Bank</rdfs:label>
    </owl:NamedIndividual>
    


    <!-- http://purl.obolibrary.org/obo/GAZ_00049753 -->

    <owl:NamedIndividual rdf:about="http://purl.obolibrary.org/obo/GAZ_00049753">
        <obo:RO_0001025 rdf:resource="http://purl.obolibrary.org/obo/GAZ_00049752"/>
        <obo:IAO_0000115>An offshore island group 51 km SSE off Morant Point, Jamaica. They consist of four small islets grouped closely together along the southeastern rim of Morant Bank a comparatively extensive crescent-shaped bank of coral, over 7 km long, rising from 1000 m.</obo:IAO_0000115>
        <oboInOwl:hasOBONamespace>GAZ</oboInOwl:hasOBONamespace>
        <oboInOwl:id>GAZ:00049753</oboInOwl:id>
        <rdfs:label>Morant Cays</rdfs:label>
    </owl:NamedIndividual>
    


    <!-- http://purl.obolibrary.org/obo/GAZ_00049754 -->

    <owl:NamedIndividual rdf:about="http://purl.obolibrary.org/obo/GAZ_00049754">
        <obo:RO_0001025 rdf:resource="http://purl.obolibrary.org/obo/GAZ_00049753"/>
        <obo:IAO_0000115>An island that lies 1.6 km southwest of South-East Cay. A rocky ledge extending from the cay is used as a pier.</obo:IAO_0000115>
        <oboInOwl:hasOBONamespace>GAZ</oboInOwl:hasOBONamespace>
        <oboInOwl:id>GAZ:00049754</oboInOwl:id>
        <rdfs:label>South-West Cay</rdfs:label>
    </owl:NamedIndividual>
    


    <!-- http://purl.obolibrary.org/obo/GAZ_00049755 -->

    <owl:NamedIndividual rdf:about="http://purl.obolibrary.org/obo/GAZ_00049755">
        <obo:RO_0001025 rdf:resource="http://purl.obolibrary.org/obo/GAZ_00049753"/>
        <obo:IAO_0000115>An island that lies 1.9 km SSW of North-East Cay. Sand spits, which extend from its ends, alter in shape with the seasons of the year; in summer the SW spit is washed away and deposited on the W side of the cay.</obo:IAO_0000115>
        <oboInOwl:hasOBONamespace>GAZ</oboInOwl:hasOBONamespace>
        <oboInOwl:id>GAZ:00049755</oboInOwl:id>
        <rdfs:label>South-East Cay</rdfs:label>
    </owl:NamedIndividual>
    


    <!-- http://purl.obolibrary.org/obo/GAZ_00049756 -->

    <owl:NamedIndividual rdf:about="http://purl.obolibrary.org/obo/GAZ_00049756">
        <obo:RO_0001025 rdf:resource="http://purl.obolibrary.org/obo/GAZ_00049753"/>
        <obo:IAO_0000115>An island that is sometimes divided into three parts, the sea washing over the connecting sand spits.</obo:IAO_0000115>
        <oboInOwl:hasOBONamespace>GAZ</oboInOwl:hasOBONamespace>
        <oboInOwl:id>GAZ:00049756</oboInOwl:id>
        <rdfs:label>North-East Cay</rdfs:label>
    </owl:NamedIndividual>
    


    <!-- http://purl.obolibrary.org/obo/GAZ_00049757 -->

    <owl:NamedIndividual rdf:about="http://purl.obolibrary.org/obo/GAZ_00049757">
        <obo:RO_0001025 rdf:resource="http://purl.obolibrary.org/obo/GAZ_00003781"/>
        <obo:IAO_0000115>A large bank of sand and coral, partially covered with seagrass, about 80 km south and southwest of Jamaica, rising steeply from a seabed of 800 meters depth. It slopes gently from Pedro Cays to the west and north with depths from 13 to 30 meters. The total area of the bank within the 100 meter isobath measures 8 040 km2. The area of a depth to 40 meters is triangular, 70 km long east-west, and 43 km wide. 2 400 km2 are less than 20 m deep.</obo:IAO_0000115>
        <oboInOwl:hasOBONamespace>GAZ</oboInOwl:hasOBONamespace>
        <oboInOwl:id>GAZ:00049757</oboInOwl:id>
        <rdfs:label>Pedro Bank</rdfs:label>
    </owl:NamedIndividual>
    


    <!-- http://purl.obolibrary.org/obo/GAZ_00049758 -->

    <owl:NamedIndividual rdf:about="http://purl.obolibrary.org/obo/GAZ_00049758">
        <obo:RO_0001025 rdf:resource="http://purl.obolibrary.org/obo/GAZ_00049757"/>
        <obo:IAO_0000115>Islands on the Pedro Bank.</obo:IAO_0000115>
        <oboInOwl:hasOBONamespace>GAZ</oboInOwl:hasOBONamespace>
        <oboInOwl:id>GAZ:00049758</oboInOwl:id>
        <rdfs:label>Pedro Cays</rdfs:label>
    </owl:NamedIndividual>
    


    <!-- http://purl.obolibrary.org/obo/GAZ_00049759 -->

    <owl:NamedIndividual rdf:about="http://purl.obolibrary.org/obo/GAZ_00049759">
        <obo:RO_0001025 rdf:resource="http://purl.obolibrary.org/obo/GAZ_00049758"/>
        <obo:IAO_0000115>An island on Pedro Bank that consists of coral and shells. This is the southernmost point of land of Jamaica.</obo:IAO_0000115>
        <oboInOwl:hasOBONamespace>GAZ</oboInOwl:hasOBONamespace>
        <oboInOwl:id>GAZ:00049759</oboInOwl:id>
        <rdfs:label>South Cay</rdfs:label>
    </owl:NamedIndividual>
    


    <!-- http://purl.obolibrary.org/obo/GAZ_00049760 -->

    <owl:NamedIndividual rdf:about="http://purl.obolibrary.org/obo/GAZ_00049760">
        <obo:RO_0001025 rdf:resource="http://purl.obolibrary.org/obo/GAZ_00049758"/>
        <obo:IAO_0000115>The largest of the Pedro Cays.</obo:IAO_0000115>
        <oboInOwl:hasOBONamespace>GAZ</oboInOwl:hasOBONamespace>
        <oboInOwl:id>GAZ:00049760</oboInOwl:id>
        <rdfs:label>Southwest Cay</rdfs:label>
    </owl:NamedIndividual>
    


    <!-- http://purl.obolibrary.org/obo/GAZ_00049761 -->

    <owl:NamedIndividual rdf:about="http://purl.obolibrary.org/obo/GAZ_00049761">
        <obo:RO_0001025 rdf:resource="http://purl.obolibrary.org/obo/GAZ_00049758"/>
        <obo:IAO_0000115>One of the Pedro Cays.</obo:IAO_0000115>
        <oboInOwl:hasOBONamespace>GAZ</oboInOwl:hasOBONamespace>
        <oboInOwl:id>GAZ:00049761</oboInOwl:id>
        <rdfs:label>Middle Cay</rdfs:label>
    </owl:NamedIndividual>
    


    <!-- http://purl.obolibrary.org/obo/GAZ_00049762 -->

    <owl:NamedIndividual rdf:about="http://purl.obolibrary.org/obo/GAZ_00049762">
        <obo:RO_0001025 rdf:resource="http://purl.obolibrary.org/obo/GAZ_00049758"/>
        <obo:IAO_0000115>One of the Pedro Cays.</obo:IAO_0000115>
        <oboInOwl:hasOBONamespace>GAZ</oboInOwl:hasOBONamespace>
        <oboInOwl:id>GAZ:00049762</oboInOwl:id>
        <rdfs:label>Northeast Cay</rdfs:label>
    </owl:NamedIndividual>
    


    <!-- http://purl.obolibrary.org/obo/GAZ_00049763 -->

    <owl:NamedIndividual rdf:about="http://purl.obolibrary.org/obo/GAZ_00049763">
        <obo:RO_0001025 rdf:resource="http://purl.obolibrary.org/obo/GAZ_00049758"/>
        <obo:IAO_0000115>A rock that lies 8 km southwest of Portland Rock, and is 0.6 m high.</obo:IAO_0000115>
        <oboInOwl:hasOBONamespace>GAZ</oboInOwl:hasOBONamespace>
        <oboInOwl:id>GAZ:00049763</oboInOwl:id>
        <rdfs:label>Blower Rock</rdfs:label>
    </owl:NamedIndividual>
    


    <!-- http://purl.obolibrary.org/obo/GAZ_00049764 -->

    <owl:NamedIndividual rdf:about="http://purl.obolibrary.org/obo/GAZ_00049764">
        <obo:RO_0001025 rdf:resource="http://purl.obolibrary.org/obo/GAZ_00049758"/>
        <obo:IAO_0000115>A rock that lies about 15 km WSW of Blower Rock. It is 0.5 m high.</obo:IAO_0000115>
        <oboInOwl:hasOBONamespace>GAZ</oboInOwl:hasOBONamespace>
        <oboInOwl:id>GAZ:00049764</oboInOwl:id>
        <rdfs:label>Shannon Rock</rdfs:label>
    </owl:NamedIndividual>
    


    <!-- http://purl.obolibrary.org/obo/GAZ_00049765 -->

    <owl:NamedIndividual rdf:about="http://purl.obolibrary.org/obo/GAZ_00049765">
        <obo:RO_0001025 rdf:resource="http://purl.obolibrary.org/obo/GAZ_00049758"/>
        <obo:IAO_0000115>A rock that lies about 63 km SSW of Portland Point, the southern extremity of Jamaica. The rock consists of two summits that lie in an east-west direction.</obo:IAO_0000115>
        <oboInOwl:hasOBONamespace>GAZ</oboInOwl:hasOBONamespace>
        <oboInOwl:id>GAZ:00049765</oboInOwl:id>
        <rdfs:label>Portland Rock</rdfs:label>
    </owl:NamedIndividual>
    


    <!-- http://purl.obolibrary.org/obo/GAZ_00049766 -->

    <owl:NamedIndividual rdf:about="http://purl.obolibrary.org/obo/GAZ_00049766">
        <obo:RO_0001025 rdf:resource="http://purl.obolibrary.org/obo/GAZ_00049757"/>
        <obo:IAO_0000115>A rock on Pedro bank with a depth of 12 m that lies 13 km northwest of Blower Rock.</obo:IAO_0000115>
        <oboInOwl:hasOBONamespace>GAZ</oboInOwl:hasOBONamespace>
        <oboInOwl:id>GAZ:00049766</oboInOwl:id>
        <rdfs:label>Willsteed Rock</rdfs:label>
    </owl:NamedIndividual>
    


    <!-- http://purl.obolibrary.org/obo/GAZ_00049767 -->

    <owl:NamedIndividual rdf:about="http://purl.obolibrary.org/obo/GAZ_00049767">
        <rdf:type rdf:resource="http://purl.obolibrary.org/obo/ENVO_00000167"/>
        <obo:RO_0001025 rdf:resource="http://purl.obolibrary.org/obo/GAZ_00049757"/>
        <obo:IAO_0000115>A shoal on Pedro Bank that has a depth of 14 m and lies 13 km NNW of Blower Rock.</obo:IAO_0000115>
        <oboInOwl:hasOBONamespace>GAZ</oboInOwl:hasOBONamespace>
        <oboInOwl:id>GAZ:00049767</oboInOwl:id>
        <rdfs:label>Doyle Shoal</rdfs:label>
    </owl:NamedIndividual>
    


    <!-- http://purl.obolibrary.org/obo/GAZ_00049768 -->

    <owl:NamedIndividual rdf:about="http://purl.obolibrary.org/obo/GAZ_00049768">
        <obo:RO_0001025 rdf:resource="http://purl.obolibrary.org/obo/GAZ_00049757"/>
        <obo:IAO_0000115>A rock on Pedro Bank that lies about 9 km southwest of Banner Reef.</obo:IAO_0000115>
        <oboInOwl:hasOBONamespace>GAZ</oboInOwl:hasOBONamespace>
        <oboInOwl:id>GAZ:00049768</oboInOwl:id>
        <rdfs:label>Southwest Rock</rdfs:label>
    </owl:NamedIndividual>
    


    <!-- http://purl.obolibrary.org/obo/GAZ_00049769 -->

    <owl:NamedIndividual rdf:about="http://purl.obolibrary.org/obo/GAZ_00049769">
        <obo:RO_0001025 rdf:resource="http://purl.obolibrary.org/obo/GAZ_00049757"/>
        <obo:IAO_0000115>A submarine feature on Pedro Bank that lies 32 km southwest of Shannon Rock, with a lowest depth of 28.8 m. It is the southernmost feature of Jamaica, not counting Alice Shoal, which is claimed by Jamaica but considered part of Colombia.</obo:IAO_0000115>
        <oboInOwl:hasOBONamespace>GAZ</oboInOwl:hasOBONamespace>
        <oboInOwl:id>GAZ:00049769</oboInOwl:id>
        <rdfs:label>Powell Knoll</rdfs:label>
    </owl:NamedIndividual>
    


    <!-- http://purl.obolibrary.org/obo/GAZ_00049770 -->

    <owl:NamedIndividual rdf:about="http://purl.obolibrary.org/obo/GAZ_00049770">
        <obo:RO_0001025 rdf:resource="http://purl.obolibrary.org/obo/GAZ_00049757"/>
        <obo:IAO_0000115>A reef on Pedro Bank that is awash. It is 2.4 km long and lies 26 km WSW of South Cay.</obo:IAO_0000115>
        <oboInOwl:hasOBONamespace>GAZ</oboInOwl:hasOBONamespace>
        <oboInOwl:id>GAZ:00049770</oboInOwl:id>
        <rdfs:label>Banner Reef</rdfs:label>
    </owl:NamedIndividual>
    


    <!-- http://purl.obolibrary.org/obo/GAZ_00049771 -->

    <owl:NamedIndividual rdf:about="http://purl.obolibrary.org/obo/GAZ_00049771">
        <obo:RO_0001025 rdf:resource="http://purl.obolibrary.org/obo/GAZ_00013512"/>
        <obo:RO_0001025 rdf:resource="http://purl.obolibrary.org/obo/GAZ_00251113"/>
        <obo:IAO_0000115>An island.</obo:IAO_0000115>
        <oboInOwl:hasOBONamespace>GAZ</oboInOwl:hasOBONamespace>
        <oboInOwl:id>GAZ:00049771</oboInOwl:id>
        <rdfs:label>Big Pelican Island</rdfs:label>
    </owl:NamedIndividual>
    


    <!-- http://purl.obolibrary.org/obo/GAZ_00049772 -->

    <owl:NamedIndividual rdf:about="http://purl.obolibrary.org/obo/GAZ_00049772">
        <obo:RO_0001025 rdf:resource="http://purl.obolibrary.org/obo/GAZ_00013508"/>
        <obo:IAO_0000115>An island.</obo:IAO_0000115>
        <oboInOwl:hasOBONamespace>GAZ</oboInOwl:hasOBONamespace>
        <oboInOwl:id>GAZ:00049772</oboInOwl:id>
        <rdfs:label>One Bush Cay</rdfs:label>
    </owl:NamedIndividual>
    


    <!-- http://purl.obolibrary.org/obo/GAZ_00049773 -->

    <owl:NamedIndividual rdf:about="http://purl.obolibrary.org/obo/GAZ_00049773">
        <obo:RO_0001025 rdf:resource="http://purl.obolibrary.org/obo/GAZ_00004339"/>
        <obo:IAO_0000115>A small island off the coast of Port Antonio in Portland Parish, Jamaica.</obo:IAO_0000115>
        <oboInOwl:hasOBONamespace>GAZ</oboInOwl:hasOBONamespace>
        <oboInOwl:id>GAZ:00049773</oboInOwl:id>
        <rdfs:label>Navy Island</rdfs:label>
    </owl:NamedIndividual>
    


    <!-- http://purl.obolibrary.org/obo/GAZ_00049774 -->

    <owl:NamedIndividual rdf:about="http://purl.obolibrary.org/obo/GAZ_00049774">
        <obo:RO_0001025 rdf:resource="http://purl.obolibrary.org/obo/GAZ_00013515"/>
        <obo:IAO_0000115>An island.</obo:IAO_0000115>
        <oboInOwl:hasOBONamespace>GAZ</oboInOwl:hasOBONamespace>
        <oboInOwl:id>GAZ:00049774</oboInOwl:id>
        <rdfs:label>Tower Island</rdfs:label>
    </owl:NamedIndividual>
    


    <!-- http://purl.obolibrary.org/obo/GAZ_00049775 -->

    <owl:NamedIndividual rdf:about="http://purl.obolibrary.org/obo/GAZ_00049775">
        <obo:RO_0001025 rdf:resource="http://purl.obolibrary.org/obo/GAZ_00013509"/>
        <obo:IAO_0000115>An island.</obo:IAO_0000115>
        <oboInOwl:hasOBONamespace>GAZ</oboInOwl:hasOBONamespace>
        <oboInOwl:id>GAZ:00049775</oboInOwl:id>
        <rdfs:label>Salt Island</rdfs:label>
    </owl:NamedIndividual>
    


    <!-- http://purl.obolibrary.org/obo/GAZ_00049776 -->

    <owl:NamedIndividual rdf:about="http://purl.obolibrary.org/obo/GAZ_00049776">
        <obo:RO_0001025 rdf:resource="http://purl.obolibrary.org/obo/GAZ_00013512"/>
        <obo:RO_0001025 rdf:resource="http://purl.obolibrary.org/obo/GAZ_00251113"/>
        <obo:IAO_0000115>An island.</obo:IAO_0000115>
        <oboInOwl:hasOBONamespace>GAZ</oboInOwl:hasOBONamespace>
        <oboInOwl:id>GAZ:00049776</oboInOwl:id>
        <rdfs:label>Pigeon Island</rdfs:label>
    </owl:NamedIndividual>
    


    <!-- http://purl.obolibrary.org/obo/GAZ_00049777 -->

    <owl:NamedIndividual rdf:about="http://purl.obolibrary.org/obo/GAZ_00049777">
        <obo:RO_0001025 rdf:resource="http://purl.obolibrary.org/obo/GAZ_00013512"/>
        <obo:RO_0001025 rdf:resource="http://purl.obolibrary.org/obo/GAZ_00251113"/>
        <obo:IAO_0000115>An island.</obo:IAO_0000115>
        <oboInOwl:hasOBONamespace>GAZ</oboInOwl:hasOBONamespace>
        <oboInOwl:id>GAZ:00049777</oboInOwl:id>
        <rdfs:label>Little Pelican Island</rdfs:label>
    </owl:NamedIndividual>
    


    <!-- http://purl.obolibrary.org/obo/GAZ_00049778 -->

    <owl:NamedIndividual rdf:about="http://purl.obolibrary.org/obo/GAZ_00049778">
        <obo:RO_0001025 rdf:resource="http://purl.obolibrary.org/obo/GAZ_00003781"/>
        <oboInOwl:hasOBONamespace>GAZ</oboInOwl:hasOBONamespace>
        <oboInOwl:id>GAZ:00049778</oboInOwl:id>
        <rdfs:label>Princess Island</rdfs:label>
    </owl:NamedIndividual>
    


    <!-- http://purl.obolibrary.org/obo/GAZ_00066432 -->

    <owl:NamedIndividual rdf:about="http://purl.obolibrary.org/obo/GAZ_00066432">
        <obo:RO_0001025 rdf:resource="http://purl.obolibrary.org/obo/GAZ_00013511"/>
        <obo:IAO_0000115>A mountain range in Saint Elizabeth Parish, Jamaica.</obo:IAO_0000115>
        <oboInOwl:hasOBONamespace>GAZ</oboInOwl:hasOBONamespace>
        <oboInOwl:id>GAZ:00066432</oboInOwl:id>
        <rdfs:label>Lacovia Mountains</rdfs:label>
    </owl:NamedIndividual>
    


    <!-- http://purl.obolibrary.org/obo/GAZ_00066433 -->

    <owl:NamedIndividual rdf:about="http://purl.obolibrary.org/obo/GAZ_00066433">
        <obo:RO_0001025 rdf:resource="http://purl.obolibrary.org/obo/GAZ_00013510"/>
        <obo:RO_0001025 rdf:resource="http://purl.obolibrary.org/obo/GAZ_00013511"/>
        <obo:IAO_0000115>A mountain range in Saint Elizabeth Parish, Jamaica.</obo:IAO_0000115>
        <oboInOwl:hasOBONamespace>GAZ</oboInOwl:hasOBONamespace>
        <oboInOwl:id>GAZ:00066433</oboInOwl:id>
        <rdfs:label>Nassau Mountains</rdfs:label>
    </owl:NamedIndividual>
    


    <!-- http://purl.obolibrary.org/obo/GAZ_00066434 -->

    <owl:NamedIndividual rdf:about="http://purl.obolibrary.org/obo/GAZ_00066434">
        <obo:RO_0001025 rdf:resource="http://purl.obolibrary.org/obo/GAZ_00013511"/>
        <obo:IAO_0000115>A mountain range in Saint Elizabeth Parish, Jamaica.</obo:IAO_0000115>
        <oboInOwl:hasOBONamespace>GAZ</oboInOwl:hasOBONamespace>
        <oboInOwl:id>GAZ:00066434</oboInOwl:id>
        <rdfs:label>Santa Cruz Mountains</rdfs:label>
    </owl:NamedIndividual>
    


    <!-- http://purl.obolibrary.org/obo/GAZ_00066435 -->

    <owl:NamedIndividual rdf:about="http://purl.obolibrary.org/obo/GAZ_00066435">
        <obo:RO_0001025 rdf:resource="http://purl.obolibrary.org/obo/GAZ_00010071"/>
        <obo:IAO_0000115>A wetland in Westmoreland Parish, Jamaica.</obo:IAO_0000115>
        <oboInOwl:hasOBONamespace>GAZ</oboInOwl:hasOBONamespace>
        <oboInOwl:id>GAZ:00066435</oboInOwl:id>
        <rdfs:label>Great Morass</rdfs:label>
    </owl:NamedIndividual>
    


    <!-- http://purl.obolibrary.org/obo/GAZ_00066436 -->

    <owl:NamedIndividual rdf:about="http://purl.obolibrary.org/obo/GAZ_00066436">
        <obo:RO_0001025 rdf:resource="http://purl.obolibrary.org/obo/GAZ_00013509"/>
        <obo:IAO_0000115>A mountain range in Clarendon Parish.</obo:IAO_0000115>
        <oboInOwl:hasOBONamespace>GAZ</oboInOwl:hasOBONamespace>
        <oboInOwl:id>GAZ:00066436</oboInOwl:id>
        <rdfs:label>Bull Head Mountain Range</rdfs:label>
    </owl:NamedIndividual>
    


    <!-- http://purl.obolibrary.org/obo/GAZ_00066437 -->

    <owl:NamedIndividual rdf:about="http://purl.obolibrary.org/obo/GAZ_00066437">
        <obo:RO_0001025 rdf:resource="http://purl.obolibrary.org/obo/GAZ_00013507"/>
        <obo:IAO_0000115>A mountain range in Manchester Parish.</obo:IAO_0000115>
        <oboInOwl:hasOBONamespace>GAZ</oboInOwl:hasOBONamespace>
        <oboInOwl:id>GAZ:00066437</oboInOwl:id>
        <rdfs:label>Carpenters Mountains</rdfs:label>
    </owl:NamedIndividual>
    


    <!-- http://purl.obolibrary.org/obo/GAZ_00066438 -->

    <owl:NamedIndividual rdf:about="http://purl.obolibrary.org/obo/GAZ_00066438">
        <obo:RO_0001025 rdf:resource="http://purl.obolibrary.org/obo/GAZ_00013507"/>
        <obo:IAO_0000115>A mountain range in Manchester Parish.</obo:IAO_0000115>
        <oboInOwl:hasOBONamespace>GAZ</oboInOwl:hasOBONamespace>
        <oboInOwl:id>GAZ:00066438</oboInOwl:id>
        <rdfs:label>May Day Mountains</rdfs:label>
    </owl:NamedIndividual>
    


    <!-- http://purl.obolibrary.org/obo/GAZ_00066439 -->

    <owl:NamedIndividual rdf:about="http://purl.obolibrary.org/obo/GAZ_00066439">
        <obo:RO_0001025 rdf:resource="http://purl.obolibrary.org/obo/GAZ_00013507"/>
        <obo:IAO_0000115>A mountain range in Manchester Parish.</obo:IAO_0000115>
        <oboInOwl:hasOBONamespace>GAZ</oboInOwl:hasOBONamespace>
        <oboInOwl:id>GAZ:00066439</oboInOwl:id>
        <rdfs:label>Don Figuerero Mountains</rdfs:label>
    </owl:NamedIndividual>
    


    <!-- http://purl.obolibrary.org/obo/GAZ_00066440 -->

    <owl:NamedIndividual rdf:about="http://purl.obolibrary.org/obo/GAZ_00066440">
        <obo:RO_0001025 rdf:resource="http://purl.obolibrary.org/obo/GAZ_00013508"/>
        <obo:IAO_0000115>A mountain range in Saint Ann Parish.</obo:IAO_0000115>
        <oboInOwl:hasOBONamespace>GAZ</oboInOwl:hasOBONamespace>
        <oboInOwl:id>GAZ:00066440</oboInOwl:id>
        <rdfs:label>Dry Harbour Mountains</rdfs:label>
    </owl:NamedIndividual>
    


    <!-- http://purl.obolibrary.org/obo/GAZ_00066441 -->

    <owl:NamedIndividual rdf:about="http://purl.obolibrary.org/obo/GAZ_00066441">
        <obo:RO_0001025 rdf:resource="http://purl.obolibrary.org/obo/GAZ_00013512"/>
        <obo:IAO_0000115>Hills in Saint Catherine Parish.</obo:IAO_0000115>
        <oboInOwl:hasOBONamespace>GAZ</oboInOwl:hasOBONamespace>
        <oboInOwl:id>GAZ:00066441</oboInOwl:id>
        <rdfs:label>Hellshire Hills</rdfs:label>
    </owl:NamedIndividual>
    


    <!-- http://purl.obolibrary.org/obo/GAZ_00066443 -->

    <owl:NamedIndividual rdf:about="http://purl.obolibrary.org/obo/GAZ_00066443">
        <obo:IAO_0000115>A national park that includes part of the Blue Mountains. Established 1992.</obo:IAO_0000115>
        <oboInOwl:hasOBONamespace>GAZ</oboInOwl:hasOBONamespace>
        <oboInOwl:id>GAZ:00066443</oboInOwl:id>
        <rdfs:label>Blue Mountain John Crow Mountain National Park</rdfs:label>
    </owl:NamedIndividual>
    


    <!-- http://purl.obolibrary.org/obo/GAZ_00066444 -->

    <owl:NamedIndividual rdf:about="http://purl.obolibrary.org/obo/GAZ_00066444">
        <obo:RO_0001025 rdf:resource="http://purl.obolibrary.org/obo/GAZ_00013513"/>
        <obo:IAO_0000115>A mountain range in Saint Thomas Parish.</obo:IAO_0000115>
        <oboInOwl:hasOBONamespace>GAZ</oboInOwl:hasOBONamespace>
        <oboInOwl:id>GAZ:00066444</oboInOwl:id>
        <rdfs:label>Port Royal Mountains</rdfs:label>
    </owl:NamedIndividual>
    


    <!-- http://purl.obolibrary.org/obo/GAZ_00066445 -->

    <owl:NamedIndividual rdf:about="http://purl.obolibrary.org/obo/GAZ_00066445">
        <obo:RO_0001025 rdf:resource="http://purl.obolibrary.org/obo/GAZ_00013513"/>
        <obo:IAO_0000115>A mountain ridge in Saint Thomas Parish.</obo:IAO_0000115>
        <oboInOwl:hasOBONamespace>GAZ</oboInOwl:hasOBONamespace>
        <oboInOwl:id>GAZ:00066445</oboInOwl:id>
        <rdfs:label>Queensbury Ridge</rdfs:label>
    </owl:NamedIndividual>
    


    <!-- http://purl.obolibrary.org/obo/GAZ_00144466 -->

    <owl:NamedIndividual rdf:about="http://purl.obolibrary.org/obo/GAZ_00144466">
        <obo:RO_0001025 rdf:resource="http://purl.obolibrary.org/obo/GAZ_00049741"/>
        <obo:IAO_0000115>A feature S of Drunkenmans Cay.</obo:IAO_0000115>
        <oboInOwl:hasOBONamespace>GAZ</oboInOwl:hasOBONamespace>
        <oboInOwl:id>GAZ:00144466</oboInOwl:id>
        <rdfs:label>South Knolls</rdfs:label>
    </owl:NamedIndividual>
    


    <!-- http://purl.obolibrary.org/obo/GAZ_00144467 -->

    <owl:NamedIndividual rdf:about="http://purl.obolibrary.org/obo/GAZ_00144467">
        <rdf:type rdf:resource="http://purl.obolibrary.org/obo/ENVO_00000167"/>
        <obo:RO_0001025 rdf:resource="http://purl.obolibrary.org/obo/GAZ_00049741"/>
        <obo:IAO_0000115>A shoal to the W of Lime Cay.</obo:IAO_0000115>
        <oboInOwl:hasOBONamespace>GAZ</oboInOwl:hasOBONamespace>
        <oboInOwl:id>GAZ:00144467</oboInOwl:id>
        <rdfs:label>Lime Cay Shoal</rdfs:label>
    </owl:NamedIndividual>
    


    <!-- http://purl.obolibrary.org/obo/GAZ_00144468 -->

    <owl:NamedIndividual rdf:about="http://purl.obolibrary.org/obo/GAZ_00144468">
        <rdf:type rdf:resource="http://purl.obolibrary.org/obo/ENVO_00000167"/>
        <obo:RO_0001025 rdf:resource="http://purl.obolibrary.org/obo/GAZ_00049741"/>
        <obo:IAO_0000115>A shoal between Drunkanmans Cay (to the W) and Maiden Cay (to the E).</obo:IAO_0000115>
        <oboInOwl:hasOBONamespace>GAZ</oboInOwl:hasOBONamespace>
        <oboInOwl:id>GAZ:00144468</oboInOwl:id>
        <rdfs:label>Biddlecombe Shoal</rdfs:label>
    </owl:NamedIndividual>
    


    <!-- http://purl.obolibrary.org/obo/GAZ_00144469 -->

    <owl:NamedIndividual rdf:about="http://purl.obolibrary.org/obo/GAZ_00144469">
        <rdf:type rdf:resource="http://purl.obolibrary.org/obo/ENVO_00000167"/>
        <obo:RO_0001025 rdf:resource="http://purl.obolibrary.org/obo/GAZ_00049741"/>
        <obo:IAO_0000115>A shoal between Maiden Cay (to the N) and Southeast Cay (to the S).</obo:IAO_0000115>
        <oboInOwl:hasOBONamespace>GAZ</oboInOwl:hasOBONamespace>
        <oboInOwl:id>GAZ:00144469</oboInOwl:id>
        <rdfs:label>East Middle Ground</rdfs:label>
    </owl:NamedIndividual>
    


    <!-- http://purl.obolibrary.org/obo/GAZ_00144470 -->

    <owl:NamedIndividual rdf:about="http://purl.obolibrary.org/obo/GAZ_00144470">
        <obo:RO_0001025 rdf:resource="http://purl.obolibrary.org/obo/GAZ_00049741"/>
        <obo:IAO_0000115>A shoal N of Drunkenmans Cay.</obo:IAO_0000115>
        <oboInOwl:hasOBONamespace>GAZ</oboInOwl:hasOBONamespace>
        <oboInOwl:id>GAZ:00144470</oboInOwl:id>
        <rdfs:label>West Middle Shoal</rdfs:label>
    </owl:NamedIndividual>
    


    <!-- http://purl.obolibrary.org/obo/GAZ_00144778 -->

    <owl:NamedIndividual rdf:about="http://purl.obolibrary.org/obo/GAZ_00144778">
        <obo:RO_0001025 rdf:resource="http://purl.obolibrary.org/obo/GAZ_00013511"/>
        <obo:IAO_0000115>A bay on the SW coast of Jamaica.</obo:IAO_0000115>
        <oboInOwl:hasOBONamespace>GAZ</oboInOwl:hasOBONamespace>
        <oboInOwl:id>GAZ:00144778</oboInOwl:id>
        <rdfs:label>Black River Bay</rdfs:label>
    </owl:NamedIndividual>
    


    <!-- http://purl.obolibrary.org/obo/GAZ_00144779 -->

    <owl:NamedIndividual rdf:about="http://purl.obolibrary.org/obo/GAZ_00144779">
        <obo:RO_0001025 rdf:resource="http://purl.obolibrary.org/obo/GAZ_00004339"/>
        <obo:IAO_0000115>The E point of Jamaica.</obo:IAO_0000115>
        <oboInOwl:hasOBONamespace>GAZ</oboInOwl:hasOBONamespace>
        <oboInOwl:id>GAZ:00144779</oboInOwl:id>
        <rdfs:label>Morant Point</rdfs:label>
    </owl:NamedIndividual>
    


    <!-- http://purl.obolibrary.org/obo/GAZ_00147866 -->

    <owl:NamedIndividual rdf:about="http://purl.obolibrary.org/obo/GAZ_00147866">
        <obo:RO_0001025 rdf:resource="http://purl.obolibrary.org/obo/GAZ_00013506"/>
        <obo:IAO_0000115>The thin tombolo of sand that serves as a natural protection for the harbour of Kingston, Jamaica.</obo:IAO_0000115>
        <oboInOwl:hasOBONamespace>GAZ</oboInOwl:hasOBONamespace>
        <oboInOwl:id>GAZ:00147866</oboInOwl:id>
        <rdfs:label>Palisadoes</rdfs:label>
    </owl:NamedIndividual>
    


    <!-- http://purl.obolibrary.org/obo/GAZ_00251084 -->

    <owl:NamedIndividual rdf:about="http://purl.obolibrary.org/obo/GAZ_00251084">
        <obo:RO_0001025 rdf:resource="http://purl.obolibrary.org/obo/GAZ_00003781"/>
        <obo:IAO_0000115>An island. One of the Greater Antilles. It is 234 km in length and as much as 80 km in width situated in the Caribbean Sea. It is about 620 km northeast of the Central American mainland, 145 km south of Cuba, and 190 kmwest of the island of Hispaniola.</obo:IAO_0000115>
        <oboInOwl:hasOBONamespace>GAZ</oboInOwl:hasOBONamespace>
        <oboInOwl:id>GAZ:00251084</oboInOwl:id>
        <rdfs:label>Jamaica</rdfs:label>
    </owl:NamedIndividual>
    


    <!-- http://purl.obolibrary.org/obo/GAZ_00251085 -->

    <owl:NamedIndividual rdf:about="http://purl.obolibrary.org/obo/GAZ_00251085">
        <obo:RO_0001025 rdf:resource="http://purl.obolibrary.org/obo/GAZ_00013510"/>
        <obo:IAO_0000115>A bay on the NW coast of Jamaica.</obo:IAO_0000115>
        <oboInOwl:hasOBONamespace>GAZ</oboInOwl:hasOBONamespace>
        <oboInOwl:id>GAZ:00251085</oboInOwl:id>
        <rdfs:label>Montego Bay</rdfs:label>
    </owl:NamedIndividual>
    


    <!-- http://purl.obolibrary.org/obo/GAZ_00251086 -->

    <owl:NamedIndividual rdf:about="http://purl.obolibrary.org/obo/GAZ_00251086">
        <obo:RO_0001025 rdf:resource="http://purl.obolibrary.org/obo/GAZ_00010070"/>
        <obo:IAO_0000115>An island.</obo:IAO_0000115>
        <oboInOwl:hasOBONamespace>GAZ</oboInOwl:hasOBONamespace>
        <oboInOwl:id>GAZ:00251086</oboInOwl:id>
        <rdfs:label>Green Island</rdfs:label>
    </owl:NamedIndividual>
    


    <!-- http://purl.obolibrary.org/obo/GAZ_00251087 -->

    <owl:NamedIndividual rdf:about="http://purl.obolibrary.org/obo/GAZ_00251087">
        <obo:RO_0001025 rdf:resource="http://purl.obolibrary.org/obo/GAZ_00013509"/>
        <obo:RO_0001025 rdf:resource="http://purl.obolibrary.org/obo/GAZ_00251113"/>
        <obo:IAO_0000115>An island.</obo:IAO_0000115>
        <oboInOwl:hasOBONamespace>GAZ</oboInOwl:hasOBONamespace>
        <oboInOwl:id>GAZ:00251087</oboInOwl:id>
        <rdfs:label>Long Island</rdfs:label>
    </owl:NamedIndividual>
    


    <!-- http://purl.obolibrary.org/obo/GAZ_00251088 -->

    <owl:NamedIndividual rdf:about="http://purl.obolibrary.org/obo/GAZ_00251088">
        <obo:RO_0001025 rdf:resource="http://purl.obolibrary.org/obo/GAZ_00013509"/>
        <obo:RO_0001025 rdf:resource="http://purl.obolibrary.org/obo/GAZ_00251113"/>
        <obo:IAO_0000115>An island.</obo:IAO_0000115>
        <oboInOwl:hasOBONamespace>GAZ</oboInOwl:hasOBONamespace>
        <oboInOwl:id>GAZ:00251088</oboInOwl:id>
        <rdfs:label>Portland Cay</rdfs:label>
    </owl:NamedIndividual>
    


    <!-- http://purl.obolibrary.org/obo/GAZ_00251089 -->

    <owl:NamedIndividual rdf:about="http://purl.obolibrary.org/obo/GAZ_00251089">
        <obo:RO_0001025 rdf:resource="http://purl.obolibrary.org/obo/GAZ_00013511"/>
        <obo:IAO_0000115>A river. The river&apos;s source is in Cockpit Country where it runs underground before emerging north of Siloah on the southern fringe Cockpits.</obo:IAO_0000115>
        <oboInOwl:hasOBONamespace>GAZ</oboInOwl:hasOBONamespace>
        <oboInOwl:id>GAZ:00251089</oboInOwl:id>
        <rdfs:label>Black River</rdfs:label>
    </owl:NamedIndividual>
    


    <!-- http://purl.obolibrary.org/obo/GAZ_00251090 -->

    <owl:NamedIndividual rdf:about="http://purl.obolibrary.org/obo/GAZ_00251090">
        <obo:RO_0001025 rdf:resource="http://purl.obolibrary.org/obo/GAZ_00251089"/>
        <obo:IAO_0000115>An island.</obo:IAO_0000115>
        <oboInOwl:hasOBONamespace>GAZ</oboInOwl:hasOBONamespace>
        <oboInOwl:id>GAZ:00251090</oboInOwl:id>
        <rdfs:label>Bore Island</rdfs:label>
    </owl:NamedIndividual>
    


    <!-- http://purl.obolibrary.org/obo/GAZ_00251091 -->

    <owl:NamedIndividual rdf:about="http://purl.obolibrary.org/obo/GAZ_00251091">
        <obo:RO_0001025 rdf:resource="http://purl.obolibrary.org/obo/GAZ_00251089"/>
        <obo:IAO_0000115>An island.</obo:IAO_0000115>
        <oboInOwl:hasOBONamespace>GAZ</oboInOwl:hasOBONamespace>
        <oboInOwl:id>GAZ:00251091</oboInOwl:id>
        <rdfs:label>Punch Island</rdfs:label>
    </owl:NamedIndividual>
    


    <!-- http://purl.obolibrary.org/obo/GAZ_00251092 -->

    <owl:NamedIndividual rdf:about="http://purl.obolibrary.org/obo/GAZ_00251092">
        <obo:RO_0001025 rdf:resource="http://purl.obolibrary.org/obo/GAZ_00251089"/>
        <obo:IAO_0000115>An island.</obo:IAO_0000115>
        <oboInOwl:hasOBONamespace>GAZ</oboInOwl:hasOBONamespace>
        <oboInOwl:id>GAZ:00251092</oboInOwl:id>
        <rdfs:label>Frenchman Island</rdfs:label>
    </owl:NamedIndividual>
    


    <!-- http://purl.obolibrary.org/obo/GAZ_00251093 -->

    <owl:NamedIndividual rdf:about="http://purl.obolibrary.org/obo/GAZ_00251093">
        <obo:RO_0001025 rdf:resource="http://purl.obolibrary.org/obo/GAZ_00013515"/>
        <obo:IAO_0000115>An island.</obo:IAO_0000115>
        <oboInOwl:hasOBONamespace>GAZ</oboInOwl:hasOBONamespace>
        <oboInOwl:id>GAZ:00251093</oboInOwl:id>
        <rdfs:label>Cabarita Island</rdfs:label>
    </owl:NamedIndividual>
    


    <!-- http://purl.obolibrary.org/obo/GAZ_00251094 -->

    <owl:NamedIndividual rdf:about="http://purl.obolibrary.org/obo/GAZ_00251094">
        <obo:RO_0001025 rdf:resource="http://purl.obolibrary.org/obo/GAZ_00013515"/>
        <obo:IAO_0000115>An island.</obo:IAO_0000115>
        <oboInOwl:hasOBONamespace>GAZ</oboInOwl:hasOBONamespace>
        <oboInOwl:id>GAZ:00251094</oboInOwl:id>
        <rdfs:label>Santa Maria Island</rdfs:label>
    </owl:NamedIndividual>
    


    <!-- http://purl.obolibrary.org/obo/GAZ_00251095 -->

    <owl:NamedIndividual rdf:about="http://purl.obolibrary.org/obo/GAZ_00251095">
        <obo:RO_0001025 rdf:resource="http://purl.obolibrary.org/obo/GAZ_00004339"/>
        <obo:IAO_0000115>An island.</obo:IAO_0000115>
        <oboInOwl:hasOBONamespace>GAZ</oboInOwl:hasOBONamespace>
        <oboInOwl:id>GAZ:00251095</oboInOwl:id>
        <rdfs:label>Pellen Island</rdfs:label>
    </owl:NamedIndividual>
    


    <!-- http://purl.obolibrary.org/obo/GAZ_00251096 -->

    <owl:NamedIndividual rdf:about="http://purl.obolibrary.org/obo/GAZ_00251096">
        <obo:RO_0001025 rdf:resource="http://purl.obolibrary.org/obo/GAZ_00004339"/>
        <obo:IAO_0000115>An island.</obo:IAO_0000115>
        <oboInOwl:hasOBONamespace>GAZ</oboInOwl:hasOBONamespace>
        <oboInOwl:id>GAZ:00251096</oboInOwl:id>
        <rdfs:label>Christmas Island</rdfs:label>
    </owl:NamedIndividual>
    


    <!-- http://purl.obolibrary.org/obo/GAZ_00251097 -->

    <owl:NamedIndividual rdf:about="http://purl.obolibrary.org/obo/GAZ_00251097">
        <obo:RO_0001025 rdf:resource="http://purl.obolibrary.org/obo/GAZ_00013512"/>
        <obo:RO_0001025 rdf:resource="http://purl.obolibrary.org/obo/GAZ_00251113"/>
        <obo:IAO_0000115>An island.</obo:IAO_0000115>
        <oboInOwl:hasOBONamespace>GAZ</oboInOwl:hasOBONamespace>
        <oboInOwl:id>GAZ:00251097</oboInOwl:id>
        <rdfs:label>Careening Island</rdfs:label>
    </owl:NamedIndividual>
    


    <!-- http://purl.obolibrary.org/obo/GAZ_00251098 -->

    <owl:NamedIndividual rdf:about="http://purl.obolibrary.org/obo/GAZ_00251098">
        <obo:RO_0001025 rdf:resource="http://purl.obolibrary.org/obo/GAZ_00013512"/>
        <obo:RO_0001025 rdf:resource="http://purl.obolibrary.org/obo/GAZ_00251113"/>
        <obo:IAO_0000115>An island.</obo:IAO_0000115>
        <oboInOwl:hasOBONamespace>GAZ</oboInOwl:hasOBONamespace>
        <oboInOwl:id>GAZ:00251098</oboInOwl:id>
        <rdfs:label>Drunkenmans Cay</rdfs:label>
    </owl:NamedIndividual>
    


    <!-- http://purl.obolibrary.org/obo/GAZ_00251099 -->

    <owl:NamedIndividual rdf:about="http://purl.obolibrary.org/obo/GAZ_00251099">
        <obo:RO_0001025 rdf:resource="http://purl.obolibrary.org/obo/GAZ_00013513"/>
        <obo:IAO_0000115>An island.</obo:IAO_0000115>
        <oboInOwl:hasOBONamespace>GAZ</oboInOwl:hasOBONamespace>
        <oboInOwl:id>GAZ:00251099</oboInOwl:id>
        <rdfs:label>Fort Island</rdfs:label>
    </owl:NamedIndividual>
    


    <!-- http://purl.obolibrary.org/obo/GAZ_00251100 -->

    <owl:NamedIndividual rdf:about="http://purl.obolibrary.org/obo/GAZ_00251100">
        <obo:RO_0001025 rdf:resource="http://purl.obolibrary.org/obo/GAZ_00013513"/>
        <obo:IAO_0000115>An island.</obo:IAO_0000115>
        <oboInOwl:hasOBONamespace>GAZ</oboInOwl:hasOBONamespace>
        <oboInOwl:id>GAZ:00251100</oboInOwl:id>
        <rdfs:label>Hogsty Cay</rdfs:label>
    </owl:NamedIndividual>
    


    <!-- http://purl.obolibrary.org/obo/GAZ_00251101 -->

    <owl:NamedIndividual rdf:about="http://purl.obolibrary.org/obo/GAZ_00251101">
        <obo:RO_0001025 rdf:resource="http://purl.obolibrary.org/obo/GAZ_00013514"/>
        <obo:IAO_0000115>An island.</obo:IAO_0000115>
        <oboInOwl:hasOBONamespace>GAZ</oboInOwl:hasOBONamespace>
        <oboInOwl:id>GAZ:00251101</oboInOwl:id>
        <rdfs:label>Bush Cay</rdfs:label>
    </owl:NamedIndividual>
    


    <!-- http://purl.obolibrary.org/obo/GAZ_00251102 -->

    <owl:NamedIndividual rdf:about="http://purl.obolibrary.org/obo/GAZ_00251102">
        <obo:RO_0001025 rdf:resource="http://purl.obolibrary.org/obo/GAZ_00013513"/>
        <obo:IAO_0000115>An island.</obo:IAO_0000115>
        <oboInOwl:hasOBONamespace>GAZ</oboInOwl:hasOBONamespace>
        <oboInOwl:id>GAZ:00251102</oboInOwl:id>
        <rdfs:label>Mango Cay</rdfs:label>
    </owl:NamedIndividual>
    


    <!-- http://purl.obolibrary.org/obo/GAZ_00251103 -->

    <owl:NamedIndividual rdf:about="http://purl.obolibrary.org/obo/GAZ_00251103">
        <obo:RO_0001025 rdf:resource="http://purl.obolibrary.org/obo/GAZ_00013513"/>
        <obo:IAO_0000115>An island.</obo:IAO_0000115>
        <oboInOwl:hasOBONamespace>GAZ</oboInOwl:hasOBONamespace>
        <oboInOwl:id>GAZ:00251103</oboInOwl:id>
        <rdfs:label>Lilyroot Cay</rdfs:label>
    </owl:NamedIndividual>
    


    <!-- http://purl.obolibrary.org/obo/GAZ_00251104 -->

    <owl:NamedIndividual rdf:about="http://purl.obolibrary.org/obo/GAZ_00251104">
        <obo:RO_0001025 rdf:resource="http://purl.obolibrary.org/obo/GAZ_00013506"/>
        <obo:IAO_0000115>An island.</obo:IAO_0000115>
        <oboInOwl:hasOBONamespace>GAZ</oboInOwl:hasOBONamespace>
        <oboInOwl:id>GAZ:00251104</oboInOwl:id>
        <rdfs:label>Maiden Cay</rdfs:label>
    </owl:NamedIndividual>
    


    <!-- http://purl.obolibrary.org/obo/GAZ_00251105 -->

    <owl:NamedIndividual rdf:about="http://purl.obolibrary.org/obo/GAZ_00251105">
        <obo:RO_0001025 rdf:resource="http://purl.obolibrary.org/obo/GAZ_00013506"/>
        <obo:IAO_0000115>An island.</obo:IAO_0000115>
        <oboInOwl:hasOBONamespace>GAZ</oboInOwl:hasOBONamespace>
        <oboInOwl:id>GAZ:00251105</oboInOwl:id>
        <rdfs:label>Gun Cay</rdfs:label>
    </owl:NamedIndividual>
    


    <!-- http://purl.obolibrary.org/obo/GAZ_00251107 -->

    <owl:NamedIndividual rdf:about="http://purl.obolibrary.org/obo/GAZ_00251107">
        <obo:RO_0001025 rdf:resource="http://purl.obolibrary.org/obo/GAZ_00013511"/>
        <obo:IAO_0000115>A wetland. Located W of the Black River. Consists of tidal mudflats, mangrove swamps and brackish marshes.</obo:IAO_0000115>
        <oboInOwl:hasOBONamespace>GAZ</oboInOwl:hasOBONamespace>
        <oboInOwl:id>GAZ:00251107</oboInOwl:id>
        <rdfs:label>Luana Swamp</rdfs:label>
    </owl:NamedIndividual>
    


    <!-- http://purl.obolibrary.org/obo/GAZ_00251108 -->

    <owl:NamedIndividual rdf:about="http://purl.obolibrary.org/obo/GAZ_00251108">
        <obo:RO_0001025 rdf:resource="http://purl.obolibrary.org/obo/GAZ_00013511"/>
        <obo:IAO_0000115>A wetland complex alonf the lower Black River. Located NE of Black River town.</obo:IAO_0000115>
        <oboInOwl:hasOBONamespace>GAZ</oboInOwl:hasOBONamespace>
        <oboInOwl:id>GAZ:00251108</oboInOwl:id>
        <rdfs:label>Black River Lower Morass</rdfs:label>
    </owl:NamedIndividual>
    


    <!-- http://purl.obolibrary.org/obo/GAZ_00251109 -->

    <owl:NamedIndividual rdf:about="http://purl.obolibrary.org/obo/GAZ_00251109">
        <obo:RO_0001025 rdf:resource="http://purl.obolibrary.org/obo/GAZ_00013511"/>
        <obo:IAO_0000115>A complex of shallow saline lagoons. Located 7 km SE of Black River.</obo:IAO_0000115>
        <oboInOwl:hasOBONamespace>GAZ</oboInOwl:hasOBONamespace>
        <oboInOwl:id>GAZ:00251109</oboInOwl:id>
        <rdfs:label>Parottee Salt Pond</rdfs:label>
    </owl:NamedIndividual>
    


    <!-- http://purl.obolibrary.org/obo/GAZ_00251110 -->

    <owl:NamedIndividual rdf:about="http://purl.obolibrary.org/obo/GAZ_00251110">
        <obo:RO_0001025 rdf:resource="http://purl.obolibrary.org/obo/GAZ_00013511"/>
        <obo:IAO_0000115>A saline lagoon. Located near Treasure Bay.</obo:IAO_0000115>
        <oboInOwl:hasOBONamespace>GAZ</oboInOwl:hasOBONamespace>
        <oboInOwl:id>GAZ:00251110</oboInOwl:id>
        <rdfs:label>Great Pedro Pond</rdfs:label>
    </owl:NamedIndividual>
    


    <!-- http://purl.obolibrary.org/obo/GAZ_00251111 -->

    <owl:NamedIndividual rdf:about="http://purl.obolibrary.org/obo/GAZ_00251111">
        <obo:RO_0001025 rdf:resource="http://purl.obolibrary.org/obo/GAZ_00013507"/>
        <obo:IAO_0000115>A wetland. A brackish marsh. Located E of Alligator Pond.</obo:IAO_0000115>
        <oboInOwl:hasOBONamespace>GAZ</oboInOwl:hasOBONamespace>
        <oboInOwl:id>GAZ:00251111</oboInOwl:id>
        <rdfs:label>Canoe Vallet</rdfs:label>
    </owl:NamedIndividual>
    


    <!-- http://purl.obolibrary.org/obo/GAZ_00251112 -->

    <owl:NamedIndividual rdf:about="http://purl.obolibrary.org/obo/GAZ_00251112">
        <obo:RO_0001025 rdf:resource="http://purl.obolibrary.org/obo/GAZ_00013509"/>
        <obo:IAO_0000115>A wetland. Located on Portland Bight. SE of Lionel Town.</obo:IAO_0000115>
        <oboInOwl:hasOBONamespace>GAZ</oboInOwl:hasOBONamespace>
        <oboInOwl:id>GAZ:00251112</oboInOwl:id>
        <rdfs:label>Portland Bight Swamp</rdfs:label>
    </owl:NamedIndividual>
    


    <!-- http://purl.obolibrary.org/obo/GAZ_00251113 -->

    <owl:NamedIndividual rdf:about="http://purl.obolibrary.org/obo/GAZ_00251113">
        <obo:IAO_0000115>A bay on the S coast of Jamaica, W of Kingston.</obo:IAO_0000115>
        <oboInOwl:hasOBONamespace>GAZ</oboInOwl:hasOBONamespace>
        <oboInOwl:id>GAZ:00251113</oboInOwl:id>
        <rdfs:label>Portland Bight</rdfs:label>
    </owl:NamedIndividual>
    


    <!-- http://purl.obolibrary.org/obo/GAZ_00251114 -->

    <owl:NamedIndividual rdf:about="http://purl.obolibrary.org/obo/GAZ_00251114">
        <obo:RO_0001025 rdf:resource="http://purl.obolibrary.org/obo/GAZ_00013509"/>
        <obo:IAO_0000115>The southernmost point in Jamaica. It is half-way along the island&apos;s south coast at the end of a hilly peninsula in Clarendon. The W limit of Portland Bight.</obo:IAO_0000115>
        <oboInOwl:hasOBONamespace>GAZ</oboInOwl:hasOBONamespace>
        <oboInOwl:id>GAZ:00251114</oboInOwl:id>
        <rdfs:label>Portland Point</rdfs:label>
    </owl:NamedIndividual>
    


    <!-- http://purl.obolibrary.org/obo/GAZ_00251115 -->

    <owl:NamedIndividual rdf:about="http://purl.obolibrary.org/obo/GAZ_00251115">
        <obo:RO_0001025 rdf:resource="http://purl.obolibrary.org/obo/GAZ_00013510"/>
        <obo:IAO_0000115>The northernmost point of mainland Jamaica. Immediately to its west is Half Moon Bay, and a little to its east is Rose Hall.</obo:IAO_0000115>
        <oboInOwl:hasOBONamespace>GAZ</oboInOwl:hasOBONamespace>
        <oboInOwl:id>GAZ:00251115</oboInOwl:id>
        <rdfs:label>Half Moon Point</rdfs:label>
    </owl:NamedIndividual>
    


    <!-- http://purl.obolibrary.org/obo/GAZ_00251116 -->

    <owl:NamedIndividual rdf:about="http://purl.obolibrary.org/obo/GAZ_00251116">
        <obo:RO_0001025 rdf:resource="http://purl.obolibrary.org/obo/GAZ_00013506"/>
        <obo:IAO_0000115>The thin tombolo of sand that serves as a natural protection for Kingston Harbour, Jamaica. Norman Manley International Airport and the historic town of Port Royal are both on Palisadoes.</obo:IAO_0000115>
        <oboInOwl:hasOBONamespace>GAZ</oboInOwl:hasOBONamespace>
        <oboInOwl:id>GAZ:00251116</oboInOwl:id>
        <rdfs:label>Palisadoes</rdfs:label>
    </owl:NamedIndividual>
    


    <!-- http://purl.obolibrary.org/obo/GAZ_00251118 -->

    <owl:NamedIndividual rdf:about="http://purl.obolibrary.org/obo/GAZ_00251118">
        <obo:RO_0001025 rdf:resource="http://purl.obolibrary.org/obo/GAZ_00010071"/>
        <obo:IAO_0000115>The westernmost point of mainland Jamaica. It is located a little south of the resort town of Negril and a little north of Negril Lighthouse.</obo:IAO_0000115>
        <oboInOwl:hasOBONamespace>GAZ</oboInOwl:hasOBONamespace>
        <oboInOwl:id>GAZ:00251118</oboInOwl:id>
        <rdfs:label>South Negril Point</rdfs:label>
    </owl:NamedIndividual>
    


    <!-- http://purl.obolibrary.org/obo/GAZ_00251119 -->

    <owl:NamedIndividual rdf:about="http://purl.obolibrary.org/obo/GAZ_00251119">
        <obo:RO_0001025 rdf:resource="http://purl.obolibrary.org/obo/GAZ_00013509"/>
        <obo:IAO_0000115>A freshwater wetland. Located E of Salt River.</obo:IAO_0000115>
        <oboInOwl:hasOBONamespace>GAZ</oboInOwl:hasOBONamespace>
        <oboInOwl:id>GAZ:00251119</oboInOwl:id>
        <rdfs:label>Cockpit-Salt River Swamp</rdfs:label>
    </owl:NamedIndividual>
    


    <!-- http://purl.obolibrary.org/obo/GAZ_00251120 -->

    <owl:NamedIndividual rdf:about="http://purl.obolibrary.org/obo/GAZ_00251120">
        <obo:RO_0001025 rdf:resource="http://purl.obolibrary.org/obo/GAZ_00013512"/>
        <obo:IAO_0000115>A wetland. Brackish lagoons behind a sand bar with tidal mudflats and mangrove swamps. Located SE of Old Harbour.</obo:IAO_0000115>
        <oboInOwl:hasOBONamespace>GAZ</oboInOwl:hasOBONamespace>
        <oboInOwl:id>GAZ:00251120</oboInOwl:id>
        <rdfs:label>Hellshire-Carabita Swamp</rdfs:label>
    </owl:NamedIndividual>
    


    <!-- http://purl.obolibrary.org/obo/GAZ_00251121 -->

    <owl:NamedIndividual rdf:about="http://purl.obolibrary.org/obo/GAZ_00251121">
        <obo:RO_0001025 rdf:resource="http://purl.obolibrary.org/obo/GAZ_00013512"/>
        <obo:IAO_0000115>A saline coastal lagoon. Now with a channel to the sea.</obo:IAO_0000115>
        <oboInOwl:hasOBONamespace>GAZ</oboInOwl:hasOBONamespace>
        <oboInOwl:id>GAZ:00251121</oboInOwl:id>
        <rdfs:label>Great Salt Pond</rdfs:label>
    </owl:NamedIndividual>
    


    <!-- http://purl.obolibrary.org/obo/GAZ_00251122 -->

    <owl:NamedIndividual rdf:about="http://purl.obolibrary.org/obo/GAZ_00251122">
        <obo:RO_0001025 rdf:resource="http://purl.obolibrary.org/obo/GAZ_00013506"/>
        <obo:IAO_0000115>A wetland. Mangrove swamps behind a sea beach. Located E of Port Royal.</obo:IAO_0000115>
        <oboInOwl:hasOBONamespace>GAZ</oboInOwl:hasOBONamespace>
        <oboInOwl:id>GAZ:00251122</oboInOwl:id>
        <rdfs:label>Port Royal Swamps</rdfs:label>
    </owl:NamedIndividual>
    


    <!-- http://purl.obolibrary.org/obo/GAZ_00251123 -->

    <owl:NamedIndividual rdf:about="http://purl.obolibrary.org/obo/GAZ_00251123">
        <obo:RO_0001025 rdf:resource="http://purl.obolibrary.org/obo/GAZ_00013513"/>
        <obo:IAO_0000115>A wetland. A mangrove swamp. Located E of Port Morant.</obo:IAO_0000115>
        <oboInOwl:hasOBONamespace>GAZ</oboInOwl:hasOBONamespace>
        <oboInOwl:id>GAZ:00251123</oboInOwl:id>
        <rdfs:label>Great Morass</rdfs:label>
    </owl:NamedIndividual>
    


    <!-- http://purl.obolibrary.org/obo/GAZ_00251124 -->

    <owl:NamedIndividual rdf:about="http://purl.obolibrary.org/obo/GAZ_00251124">
        <obo:RO_0001025 rdf:resource="http://purl.obolibrary.org/obo/GAZ_00004339"/>
        <obo:IAO_0000115>A wetland. A mangrove swamp and tidal marshes behind a sea beach. Located E of Port Antonio.</obo:IAO_0000115>
        <oboInOwl:hasOBONamespace>GAZ</oboInOwl:hasOBONamespace>
        <oboInOwl:id>GAZ:00251124</oboInOwl:id>
        <rdfs:label>Turtle Crawle Swamp</rdfs:label>
    </owl:NamedIndividual>
    


    <!-- http://purl.obolibrary.org/obo/GAZ_00251125 -->

    <owl:NamedIndividual rdf:about="http://purl.obolibrary.org/obo/GAZ_00251125">
        <obo:RO_0001025 rdf:resource="http://purl.obolibrary.org/obo/GAZ_00013508"/>
        <obo:IAO_0000115>A freshwater wetland. A springfed marsh with clear pools behind a sea beach. Located E of Runaway Bay.</obo:IAO_0000115>
        <oboInOwl:hasOBONamespace>GAZ</oboInOwl:hasOBONamespace>
        <oboInOwl:id>GAZ:00251125</oboInOwl:id>
        <rdfs:label>Pear Tree Swamp</rdfs:label>
    </owl:NamedIndividual>
    


    <!-- http://purl.obolibrary.org/obo/GAZ_00251126 -->

    <owl:NamedIndividual rdf:about="http://purl.obolibrary.org/obo/GAZ_00251126">
        <obo:RO_0001025 rdf:resource="http://purl.obolibrary.org/obo/GAZ_00010071"/>
        <obo:IAO_0000115>A bay. Located N of Negril.</obo:IAO_0000115>
        <oboInOwl:hasOBONamespace>GAZ</oboInOwl:hasOBONamespace>
        <oboInOwl:id>GAZ:00251126</oboInOwl:id>
        <rdfs:label>Orange Bay [Westmoreland]</rdfs:label>
    </owl:NamedIndividual>
    


    <!-- http://purl.obolibrary.org/obo/GAZ_00251127 -->

    <owl:NamedIndividual rdf:about="http://purl.obolibrary.org/obo/GAZ_00251127">
        <obo:RO_0001025 rdf:resource="http://purl.obolibrary.org/obo/GAZ_00004339"/>
        <obo:IAO_0000115>A bay. Located 15 miles W of Port Antonio.</obo:IAO_0000115>
        <oboInOwl:hasOBONamespace>GAZ</oboInOwl:hasOBONamespace>
        <oboInOwl:id>GAZ:00251127</oboInOwl:id>
        <rdfs:label>Orange Bay [Portland]</rdfs:label>
    </owl:NamedIndividual>
    


    <!-- http://purl.obolibrary.org/obo/GAZ_00251128 -->

    <owl:NamedIndividual rdf:about="http://purl.obolibrary.org/obo/GAZ_00251128">
        <obo:RO_0001025 rdf:resource="http://purl.obolibrary.org/obo/GAZ_00010072"/>
        <obo:IAO_0000115>A cove on the cliffs of Negril, in Westmoreland, Jamaica. It consists of a labyrinth of caves and passageways carved from solid rock.</obo:IAO_0000115>
        <oboInOwl:hasOBONamespace>GAZ</oboInOwl:hasOBONamespace>
        <oboInOwl:id>GAZ:00251128</oboInOwl:id>
        <rdfs:label>Xtabi</rdfs:label>
    </owl:NamedIndividual>
    


    <!-- http://purl.obolibrary.org/obo/GAZ_00251129 -->

    <owl:NamedIndividual rdf:about="http://purl.obolibrary.org/obo/GAZ_00251129">
        <obo:RO_0001025 rdf:resource="http://purl.obolibrary.org/obo/GAZ_00251147"/>
        <obo:IAO_0000115>A karst cave in the Cockpit Country of Jamaica.</obo:IAO_0000115>
        <oboInOwl:hasOBONamespace>GAZ</oboInOwl:hasOBONamespace>
        <oboInOwl:id>GAZ:00251129</oboInOwl:id>
        <rdfs:label>Bad Hole Cave</rdfs:label>
    </owl:NamedIndividual>
    


    <!-- http://purl.obolibrary.org/obo/GAZ_00251130 -->

    <owl:NamedIndividual rdf:about="http://purl.obolibrary.org/obo/GAZ_00251130">
        <obo:RO_0001025 rdf:resource="http://purl.obolibrary.org/obo/GAZ_00251147"/>
        <obo:IAO_0000115>A dry karst cave in the Cockpit Country of Jamaica.</obo:IAO_0000115>
        <oboInOwl:hasOBONamespace>GAZ</oboInOwl:hasOBONamespace>
        <oboInOwl:id>GAZ:00251130</oboInOwl:id>
        <rdfs:label>Belmont Cave</rdfs:label>
    </owl:NamedIndividual>
    


    <!-- http://purl.obolibrary.org/obo/GAZ_00251131 -->

    <owl:NamedIndividual rdf:about="http://purl.obolibrary.org/obo/GAZ_00251131">
        <obo:RO_0001025 rdf:resource="http://purl.obolibrary.org/obo/GAZ_00251147"/>
        <obo:IAO_0000115>A dry karst cave in Trelawny, Jamaica.</obo:IAO_0000115>
        <oboInOwl:hasOBONamespace>GAZ</oboInOwl:hasOBONamespace>
        <oboInOwl:id>GAZ:00251131</oboInOwl:id>
        <rdfs:label>Carambie Cave</rdfs:label>
    </owl:NamedIndividual>
    


    <!-- http://purl.obolibrary.org/obo/GAZ_00251132 -->

    <owl:NamedIndividual rdf:about="http://purl.obolibrary.org/obo/GAZ_00251132">
        <obo:RO_0001025 rdf:resource="http://purl.obolibrary.org/obo/GAZ_00013507"/>
        <obo:IAO_0000115>A large river cave in Manchester Parish in west-central Jamaica. It is 2800 m in length and at an altitude of 250 m.</obo:IAO_0000115>
        <oboInOwl:hasOBONamespace>GAZ</oboInOwl:hasOBONamespace>
        <oboInOwl:id>GAZ:00251132</oboInOwl:id>
        <rdfs:label>Coffee River Cave</rdfs:label>
    </owl:NamedIndividual>
    


    <!-- http://purl.obolibrary.org/obo/GAZ_00251133 -->

    <owl:NamedIndividual rdf:about="http://purl.obolibrary.org/obo/GAZ_00251133">
        <obo:RO_0001025 rdf:resource="http://purl.obolibrary.org/obo/GAZ_00251147"/>
        <obo:IAO_0000115>A karst cave. A large chamber cave in Trelawny, Jamaica.</obo:IAO_0000115>
        <oboInOwl:hasOBONamespace>GAZ</oboInOwl:hasOBONamespace>
        <oboInOwl:id>GAZ:00251133</oboInOwl:id>
        <rdfs:label>Dunn&apos;s Hole</rdfs:label>
    </owl:NamedIndividual>
    


    <!-- http://purl.obolibrary.org/obo/GAZ_00251134 -->

    <owl:NamedIndividual rdf:about="http://purl.obolibrary.org/obo/GAZ_00251134">
        <obo:RO_0001025 rdf:resource="http://purl.obolibrary.org/obo/GAZ_00013507"/>
        <obo:IAO_0000115>A river cave in Manchester Parish in west-central Jamaica.</obo:IAO_0000115>
        <oboInOwl:hasOBONamespace>GAZ</oboInOwl:hasOBONamespace>
        <oboInOwl:id>GAZ:00251134</oboInOwl:id>
        <rdfs:label>Gourie Cave</rdfs:label>
    </owl:NamedIndividual>
    


    <!-- http://purl.obolibrary.org/obo/GAZ_00251135 -->

    <owl:NamedIndividual rdf:about="http://purl.obolibrary.org/obo/GAZ_00251135">
        <rdf:type rdf:resource="http://purl.obolibrary.org/obo/ENVO_00000856"/>
        <obo:RO_0001025 rdf:resource="http://purl.obolibrary.org/obo/GAZ_00013508"/>
        <obo:IAO_0000115>A populated place. A town in Saint Ann Parish on the northern coast of Jamaica.</obo:IAO_0000115>
        <oboInOwl:hasOBONamespace>GAZ</oboInOwl:hasOBONamespace>
        <oboInOwl:id>GAZ:00251135</oboInOwl:id>
        <rdfs:label>Discovery Bay</rdfs:label>
    </owl:NamedIndividual>
    


    <!-- http://purl.obolibrary.org/obo/GAZ_00251136 -->

    <owl:NamedIndividual rdf:about="http://purl.obolibrary.org/obo/GAZ_00251136">
        <obo:RO_0001025 rdf:resource="http://purl.obolibrary.org/obo/GAZ_00251135"/>
        <obo:IAO_0000115>Show caves in Discovery Bay, Saint Ann on the north coast of Jamaica. Tidal cut.</obo:IAO_0000115>
        <oboInOwl:hasOBONamespace>GAZ</oboInOwl:hasOBONamespace>
        <oboInOwl:id>GAZ:00251136</oboInOwl:id>
        <rdfs:label>Green Grotto Caves</rdfs:label>
    </owl:NamedIndividual>
    


    <!-- http://purl.obolibrary.org/obo/GAZ_00251137 -->

    <owl:NamedIndividual rdf:about="http://purl.obolibrary.org/obo/GAZ_00251137">
        <obo:RO_0001025 rdf:resource="http://purl.obolibrary.org/obo/GAZ_00013508"/>
        <obo:IAO_0000115>A large sinkhole located in Saint Ann in northern Jamaica.</obo:IAO_0000115>
        <oboInOwl:hasOBONamespace>GAZ</oboInOwl:hasOBONamespace>
        <oboInOwl:id>GAZ:00251137</oboInOwl:id>
        <rdfs:label>Hutchinson&apos;s Hole</rdfs:label>
    </owl:NamedIndividual>
    


    <!-- http://purl.obolibrary.org/obo/GAZ_00251138 -->

    <owl:NamedIndividual rdf:about="http://purl.obolibrary.org/obo/GAZ_00251138">
        <obo:RO_0001025 rdf:resource="http://purl.obolibrary.org/obo/GAZ_00013509"/>
        <obo:IAO_0000115>A very large cave system on the Portland Ridge in Clarendon near the south coast of Jamaica.</obo:IAO_0000115>
        <oboInOwl:hasOBONamespace>GAZ</oboInOwl:hasOBONamespace>
        <oboInOwl:id>GAZ:00251138</oboInOwl:id>
        <rdfs:label>Jackson&apos;s Bay Cave</rdfs:label>
    </owl:NamedIndividual>
    


    <!-- http://purl.obolibrary.org/obo/GAZ_00251139 -->

    <owl:NamedIndividual rdf:about="http://purl.obolibrary.org/obo/GAZ_00251139">
        <obo:RO_0001025 rdf:resource="http://purl.obolibrary.org/obo/GAZ_00013507"/>
        <obo:IAO_0000115>A cave.</obo:IAO_0000115>
        <oboInOwl:hasOBONamespace>GAZ</oboInOwl:hasOBONamespace>
        <oboInOwl:id>GAZ:00251139</oboInOwl:id>
        <rdfs:label>Morgans Pond Hole</rdfs:label>
    </owl:NamedIndividual>
    


    <!-- http://purl.obolibrary.org/obo/GAZ_00251140 -->

    <owl:NamedIndividual rdf:about="http://purl.obolibrary.org/obo/GAZ_00251140">
        <obo:RO_0001025 rdf:resource="http://purl.obolibrary.org/obo/GAZ_00251147"/>
        <obo:IAO_0000115>A large, labyrinthine river cave in Trelawny, Jamaica. It is the only exit of the Mouth River.</obo:IAO_0000115>
        <oboInOwl:hasOBONamespace>GAZ</oboInOwl:hasOBONamespace>
        <oboInOwl:id>GAZ:00251140</oboInOwl:id>
        <rdfs:label>Mouth Maze Cave</rdfs:label>
    </owl:NamedIndividual>
    


    <!-- http://purl.obolibrary.org/obo/GAZ_00251141 -->

    <owl:NamedIndividual rdf:about="http://purl.obolibrary.org/obo/GAZ_00251141">
        <obo:RO_0001025 rdf:resource="http://purl.obolibrary.org/obo/GAZ_00013507"/>
        <obo:IAO_0000115>A cave in Manchester Parish in west-central Jamaica.</obo:IAO_0000115>
        <oboInOwl:hasOBONamespace>GAZ</oboInOwl:hasOBONamespace>
        <oboInOwl:id>GAZ:00251141</oboInOwl:id>
        <rdfs:label>Oxford Cave</rdfs:label>
    </owl:NamedIndividual>
    


    <!-- http://purl.obolibrary.org/obo/GAZ_00251142 -->

    <owl:NamedIndividual rdf:about="http://purl.obolibrary.org/obo/GAZ_00251142">
        <obo:RO_0001025 rdf:resource="http://purl.obolibrary.org/obo/GAZ_00013507"/>
        <obo:IAO_0000115>A cave.</obo:IAO_0000115>
        <oboInOwl:hasOBONamespace>GAZ</oboInOwl:hasOBONamespace>
        <oboInOwl:id>GAZ:00251142</oboInOwl:id>
        <rdfs:label>Smokey Hole Cave</rdfs:label>
    </owl:NamedIndividual>
    


    <!-- http://purl.obolibrary.org/obo/GAZ_00251143 -->

    <owl:NamedIndividual rdf:about="http://purl.obolibrary.org/obo/GAZ_00251143">
        <obo:RO_0001025 rdf:resource="http://purl.obolibrary.org/obo/GAZ_00013508"/>
        <obo:IAO_0000115>A large cave in St Ann near the north coast of Jamaica.</obo:IAO_0000115>
        <oboInOwl:hasOBONamespace>GAZ</oboInOwl:hasOBONamespace>
        <oboInOwl:id>GAZ:00251143</oboInOwl:id>
        <rdfs:label>Thatchfield Great Cave</rdfs:label>
    </owl:NamedIndividual>
    


    <!-- http://purl.obolibrary.org/obo/GAZ_00251144 -->

    <owl:NamedIndividual rdf:about="http://purl.obolibrary.org/obo/GAZ_00251144">
        <obo:RO_0001025 rdf:resource="http://purl.obolibrary.org/obo/GAZ_00251147"/>
        <obo:IAO_0000115>A 3,000 m long complex of linked caves in Trelawny Parish on the north coast of Jamaica.</obo:IAO_0000115>
        <oboInOwl:hasOBONamespace>GAZ</oboInOwl:hasOBONamespace>
        <oboInOwl:id>GAZ:00251144</oboInOwl:id>
        <rdfs:label>Windsor Great Cave</rdfs:label>
    </owl:NamedIndividual>
    


    <!-- http://purl.obolibrary.org/obo/GAZ_00251145 -->

    <owl:NamedIndividual rdf:about="http://purl.obolibrary.org/obo/GAZ_00251145">
        <rdf:type rdf:resource="http://purl.obolibrary.org/obo/ENVO_00000106"/>
        <obo:RO_0001025 rdf:resource="http://purl.obolibrary.org/obo/GAZ_00004339"/>
        <obo:IAO_0000115>A range of mountains in Jamaica. They extend parallel with the short eastern coast of the island, bounded to the west by the banks of the Rio Grande, and joining with the eastern end of the Blue Mountains in the south.</obo:IAO_0000115>
        <oboInOwl:hasOBONamespace>GAZ</oboInOwl:hasOBONamespace>
        <oboInOwl:id>GAZ:00251145</oboInOwl:id>
        <rdfs:label>John Crow Mountains</rdfs:label>
    </owl:NamedIndividual>
    


    <!-- http://purl.obolibrary.org/obo/GAZ_00251146 -->

    <owl:NamedIndividual rdf:about="http://purl.obolibrary.org/obo/GAZ_00251146">
        <obo:RO_0001025 rdf:resource="http://purl.obolibrary.org/obo/GAZ_00013509"/>
        <obo:IAO_0000115>A mountain range in south central Jamaica.</obo:IAO_0000115>
        <oboInOwl:hasOBONamespace>GAZ</oboInOwl:hasOBONamespace>
        <oboInOwl:id>GAZ:00251146</oboInOwl:id>
        <rdfs:label>Mocho Mountains</rdfs:label>
    </owl:NamedIndividual>
    


    <!-- http://purl.obolibrary.org/obo/GAZ_00251147 -->

    <owl:NamedIndividual rdf:about="http://purl.obolibrary.org/obo/GAZ_00251147">
        <rdf:type rdf:resource="http://purl.obolibrary.org/obo/ENVO_00000175"/>
        <obo:RO_0001025 rdf:resource="http://purl.obolibrary.org/obo/GAZ_00013514"/>
        <obo:IAO_0000115>A karst area in Jamaica.</obo:IAO_0000115>
        <oboInOwl:hasOBONamespace>GAZ</oboInOwl:hasOBONamespace>
        <oboInOwl:id>GAZ:00251147</oboInOwl:id>
        <rdfs:label>Cockpit Country</rdfs:label>
    </owl:NamedIndividual>
    


    <!-- http://purl.obolibrary.org/obo/GAZ_00251148 -->

    <owl:NamedIndividual rdf:about="http://purl.obolibrary.org/obo/GAZ_00251148">
        <obo:RO_0001025 rdf:resource="http://purl.obolibrary.org/obo/GAZ_00251147"/>
        <obo:IAO_0000115>A valley.</obo:IAO_0000115>
        <oboInOwl:hasOBONamespace>GAZ</oboInOwl:hasOBONamespace>
        <oboInOwl:id>GAZ:00251148</oboInOwl:id>
        <rdfs:label>Vale of Clarendon</rdfs:label>
    </owl:NamedIndividual>
    


    <!-- http://purl.obolibrary.org/obo/GAZ_00251149 -->

    <owl:NamedIndividual rdf:about="http://purl.obolibrary.org/obo/GAZ_00251149">
        <obo:RO_0001025 rdf:resource="http://purl.obolibrary.org/obo/GAZ_00251147"/>
        <obo:IAO_0000115>A valley.</obo:IAO_0000115>
        <oboInOwl:hasOBONamespace>GAZ</oboInOwl:hasOBONamespace>
        <oboInOwl:id>GAZ:00251149</oboInOwl:id>
        <rdfs:label>Queen of Spains Valley</rdfs:label>
    </owl:NamedIndividual>
    


    <!-- http://purl.obolibrary.org/obo/GAZ_00251150 -->

    <owl:NamedIndividual rdf:about="http://purl.obolibrary.org/obo/GAZ_00251150">
        <obo:RO_0001025 rdf:resource="http://purl.obolibrary.org/obo/GAZ_00251147"/>
        <obo:IAO_0000115>A valley.</obo:IAO_0000115>
        <oboInOwl:hasOBONamespace>GAZ</oboInOwl:hasOBONamespace>
        <oboInOwl:id>GAZ:00251150</oboInOwl:id>
        <rdfs:label>Nassau Valley</rdfs:label>
    </owl:NamedIndividual>
    


    <!-- http://purl.obolibrary.org/obo/GAZ_00251151 -->

    <owl:NamedIndividual rdf:about="http://purl.obolibrary.org/obo/GAZ_00251151">
        <obo:RO_0001025 rdf:resource="http://purl.obolibrary.org/obo/GAZ_00251147"/>
        <oboInOwl:hasOBONamespace>GAZ</oboInOwl:hasOBONamespace>
        <oboInOwl:id>GAZ:00251151</oboInOwl:id>
        <rdfs:label>Cave Valley</rdfs:label>
    </owl:NamedIndividual>
    


    <!-- http://purl.obolibrary.org/obo/GAZ_00251152 -->

    <owl:NamedIndividual rdf:about="http://purl.obolibrary.org/obo/GAZ_00251152">
        <obo:RO_0001025 rdf:resource="http://purl.obolibrary.org/obo/GAZ_00010071"/>
        <obo:IAO_0000115>A river.</obo:IAO_0000115>
        <oboInOwl:hasOBONamespace>GAZ</oboInOwl:hasOBONamespace>
        <oboInOwl:id>GAZ:00251152</oboInOwl:id>
        <rdfs:label>South Negril River</rdfs:label>
    </owl:NamedIndividual>
    


    <!-- http://purl.obolibrary.org/obo/GAZ_00251153 -->

    <owl:NamedIndividual rdf:about="http://purl.obolibrary.org/obo/GAZ_00251153">
        <obo:RO_0001025 rdf:resource="http://purl.obolibrary.org/obo/GAZ_00010071"/>
        <obo:IAO_0000115>A river.</obo:IAO_0000115>
        <oboInOwl:hasOBONamespace>GAZ</oboInOwl:hasOBONamespace>
        <oboInOwl:id>GAZ:00251153</oboInOwl:id>
        <rdfs:label>North Negril River</rdfs:label>
    </owl:NamedIndividual>
    


    <!-- http://purl.obolibrary.org/obo/GAZ_00251154 -->

    <owl:NamedIndividual rdf:about="http://purl.obolibrary.org/obo/GAZ_00251154">
        <obo:RO_0001025 rdf:resource="http://purl.obolibrary.org/obo/GAZ_00013507"/>
        <obo:IAO_0000115>A river.</obo:IAO_0000115>
        <oboInOwl:hasOBONamespace>GAZ</oboInOwl:hasOBONamespace>
        <oboInOwl:id>GAZ:00251154</oboInOwl:id>
        <rdfs:label>Alligator Hole River</rdfs:label>
    </owl:NamedIndividual>
    


    <!-- http://purl.obolibrary.org/obo/GAZ_00251155 -->

    <owl:NamedIndividual rdf:about="http://purl.obolibrary.org/obo/GAZ_00251155">
        <obo:RO_0001025 rdf:resource="http://purl.obolibrary.org/obo/GAZ_00013515"/>
        <obo:IAO_0000115>A river.</obo:IAO_0000115>
        <oboInOwl:hasOBONamespace>GAZ</oboInOwl:hasOBONamespace>
        <oboInOwl:id>GAZ:00251155</oboInOwl:id>
        <rdfs:label>Annotto River</rdfs:label>
    </owl:NamedIndividual>
    


    <!-- http://purl.obolibrary.org/obo/GAZ_00251156 -->

    <owl:NamedIndividual rdf:about="http://purl.obolibrary.org/obo/GAZ_00251156">
        <obo:RO_0001025 rdf:resource="http://purl.obolibrary.org/obo/GAZ_00251155"/>
        <obo:IAO_0000115>A river.</obo:IAO_0000115>
        <oboInOwl:hasOBONamespace>GAZ</oboInOwl:hasOBONamespace>
        <oboInOwl:id>GAZ:00251156</oboInOwl:id>
        <rdfs:label>New Savannah River</rdfs:label>
    </owl:NamedIndividual>
    


    <!-- http://purl.obolibrary.org/obo/GAZ_00251157 -->

    <owl:NamedIndividual rdf:about="http://purl.obolibrary.org/obo/GAZ_00251157">
        <obo:RO_0001025 rdf:resource="http://purl.obolibrary.org/obo/GAZ_00010071"/>
        <obo:IAO_0000115>A river.</obo:IAO_0000115>
        <oboInOwl:hasOBONamespace>GAZ</oboInOwl:hasOBONamespace>
        <oboInOwl:id>GAZ:00251157</oboInOwl:id>
        <rdfs:label>Cabarita River</rdfs:label>
    </owl:NamedIndividual>
    


    <!-- http://purl.obolibrary.org/obo/GAZ_00251160 -->

    <owl:NamedIndividual rdf:about="http://purl.obolibrary.org/obo/GAZ_00251160">
        <obo:RO_0001025 rdf:resource="http://purl.obolibrary.org/obo/GAZ_00010071"/>
        <obo:IAO_0000115>A river.</obo:IAO_0000115>
        <oboInOwl:hasOBONamespace>GAZ</oboInOwl:hasOBONamespace>
        <oboInOwl:id>GAZ:00251160</oboInOwl:id>
        <rdfs:label>Sweet River</rdfs:label>
    </owl:NamedIndividual>
    


    <!-- http://purl.obolibrary.org/obo/GAZ_00251161 -->

    <owl:NamedIndividual rdf:about="http://purl.obolibrary.org/obo/GAZ_00251161">
        <obo:RO_0001025 rdf:resource="http://purl.obolibrary.org/obo/GAZ_00013511"/>
        <obo:IAO_0000115>A river.</obo:IAO_0000115>
        <oboInOwl:hasOBONamespace>GAZ</oboInOwl:hasOBONamespace>
        <oboInOwl:id>GAZ:00251161</oboInOwl:id>
        <rdfs:label>Broad River</rdfs:label>
    </owl:NamedIndividual>
    


    <!-- http://purl.obolibrary.org/obo/GAZ_00251162 -->

    <owl:NamedIndividual rdf:about="http://purl.obolibrary.org/obo/GAZ_00251162">
        <obo:RO_0001025 rdf:resource="http://purl.obolibrary.org/obo/GAZ_00013511"/>
        <obo:IAO_0000115>A river.</obo:IAO_0000115>
        <oboInOwl:hasOBONamespace>GAZ</oboInOwl:hasOBONamespace>
        <oboInOwl:id>GAZ:00251162</oboInOwl:id>
        <rdfs:label>Y.S. River</rdfs:label>
    </owl:NamedIndividual>
    


    <!-- http://purl.obolibrary.org/obo/GAZ_00251163 -->

    <owl:NamedIndividual rdf:about="http://purl.obolibrary.org/obo/GAZ_00251163">
        <obo:RO_0001025 rdf:resource="http://purl.obolibrary.org/obo/GAZ_00013511"/>
        <obo:IAO_0000115>A river.</obo:IAO_0000115>
        <oboInOwl:hasOBONamespace>GAZ</oboInOwl:hasOBONamespace>
        <oboInOwl:id>GAZ:00251163</oboInOwl:id>
        <rdfs:label>Smith River</rdfs:label>
    </owl:NamedIndividual>
    


    <!-- http://purl.obolibrary.org/obo/GAZ_00251166 -->

    <owl:NamedIndividual rdf:about="http://purl.obolibrary.org/obo/GAZ_00251166">
        <obo:RO_0001025 rdf:resource="http://purl.obolibrary.org/obo/GAZ_00013507"/>
        <obo:IAO_0000115>A river. It rises to the south-west of Comfort Hall, a small village, and flows south, then west then north in a large loop through the hamlet of Dick or Duck Pond, which brings it back to the same latitude it started from before heading generally north-west to its confluence with the One Eye River.</obo:IAO_0000115>
        <oboInOwl:hasOBONamespace>GAZ</oboInOwl:hasOBONamespace>
        <oboInOwl:id>GAZ:00251166</oboInOwl:id>
        <rdfs:label>Rotten Gut River</rdfs:label>
    </owl:NamedIndividual>
    


    <!-- http://purl.obolibrary.org/obo/GAZ_00251167 -->

    <owl:NamedIndividual rdf:about="http://purl.obolibrary.org/obo/GAZ_00251167">
        <obo:RO_0001025 rdf:resource="http://purl.obolibrary.org/obo/GAZ_00013507"/>
        <obo:IAO_0000115>A river. Mostly underground, it springs forth in a deep clear pool barely 200m from the sea.</obo:IAO_0000115>
        <oboInOwl:hasOBONamespace>GAZ</oboInOwl:hasOBONamespace>
        <oboInOwl:id>GAZ:00251167</oboInOwl:id>
        <rdfs:label>Gut River</rdfs:label>
    </owl:NamedIndividual>
    


    <!-- http://purl.obolibrary.org/obo/GAZ_00251168 -->

    <owl:NamedIndividual rdf:about="http://purl.obolibrary.org/obo/GAZ_00251168">
        <obo:RO_0001025 rdf:resource="http://purl.obolibrary.org/obo/GAZ_00013509"/>
        <obo:IAO_0000115>A river.</obo:IAO_0000115>
        <oboInOwl:hasOBONamespace>GAZ</oboInOwl:hasOBONamespace>
        <oboInOwl:id>GAZ:00251168</oboInOwl:id>
        <rdfs:label>Milk River</rdfs:label>
    </owl:NamedIndividual>
    


    <!-- http://purl.obolibrary.org/obo/GAZ_00251169 -->

    <owl:NamedIndividual rdf:about="http://purl.obolibrary.org/obo/GAZ_00251169">
        <obo:RO_0001025 rdf:resource="http://purl.obolibrary.org/obo/GAZ_00013509"/>
        <obo:IAO_0000115>A river that flows generally south-southwest and reaches the Caribbean Sea at Carlisle Bay in the central south coast, to the west of the island&apos;s southernmost point, Portland Point.</obo:IAO_0000115>
        <oboInOwl:hasOBONamespace>GAZ</oboInOwl:hasOBONamespace>
        <oboInOwl:id>GAZ:00251169</oboInOwl:id>
        <rdfs:label>Rio Minho</rdfs:label>
    </owl:NamedIndividual>
    


    <!-- http://purl.obolibrary.org/obo/GAZ_00251170 -->

    <owl:NamedIndividual rdf:about="http://purl.obolibrary.org/obo/GAZ_00251170">
        <obo:RO_0001025 rdf:resource="http://purl.obolibrary.org/obo/GAZ_00010071"/>
        <obo:IAO_0000115>A river.</obo:IAO_0000115>
        <oboInOwl:hasOBONamespace>GAZ</oboInOwl:hasOBONamespace>
        <oboInOwl:id>GAZ:00251170</oboInOwl:id>
        <rdfs:label>Salt River</rdfs:label>
    </owl:NamedIndividual>
    


    <!-- http://purl.obolibrary.org/obo/GAZ_00251171 -->

    <owl:NamedIndividual rdf:about="http://purl.obolibrary.org/obo/GAZ_00251171">
        <obo:RO_0001025 rdf:resource="http://purl.obolibrary.org/obo/GAZ_00013512"/>
        <obo:IAO_0000115>A river.</obo:IAO_0000115>
        <oboInOwl:hasOBONamespace>GAZ</oboInOwl:hasOBONamespace>
        <oboInOwl:id>GAZ:00251171</oboInOwl:id>
        <rdfs:label>Coleburns Gully</rdfs:label>
    </owl:NamedIndividual>
    


    <!-- http://purl.obolibrary.org/obo/GAZ_00251172 -->

    <owl:NamedIndividual rdf:about="http://purl.obolibrary.org/obo/GAZ_00251172">
        <obo:RO_0001025 rdf:resource="http://purl.obolibrary.org/obo/GAZ_00013512"/>
        <obo:IAO_0000115>A river. Its source is unclear. It flows to meet the Caribbean Sea in the north west corner of Kingston Harbour.</obo:IAO_0000115>
        <oboInOwl:hasOBONamespace>GAZ</oboInOwl:hasOBONamespace>
        <oboInOwl:id>GAZ:00251172</oboInOwl:id>
        <rdfs:label>Rio Cobre</rdfs:label>
    </owl:NamedIndividual>
    


    <!-- http://purl.obolibrary.org/obo/GAZ_00251173 -->

    <owl:NamedIndividual rdf:about="http://purl.obolibrary.org/obo/GAZ_00251173">
        <obo:IAO_0000115>A bay.</obo:IAO_0000115>
        <oboInOwl:hasOBONamespace>GAZ</oboInOwl:hasOBONamespace>
        <oboInOwl:id>GAZ:00251173</oboInOwl:id>
        <rdfs:label>Hunts Bay</rdfs:label>
    </owl:NamedIndividual>
    


    <!-- http://purl.obolibrary.org/obo/GAZ_00251177 -->

    <owl:NamedIndividual rdf:about="http://purl.obolibrary.org/obo/GAZ_00251177">
        <obo:RO_0001025 rdf:resource="http://purl.obolibrary.org/obo/GAZ_00013512"/>
        <obo:IAO_0000115>A river.</obo:IAO_0000115>
        <oboInOwl:hasOBONamespace>GAZ</oboInOwl:hasOBONamespace>
        <oboInOwl:id>GAZ:00251177</oboInOwl:id>
        <rdfs:label>Fresh River</rdfs:label>
    </owl:NamedIndividual>
    


    <!-- http://purl.obolibrary.org/obo/GAZ_00251178 -->

    <owl:NamedIndividual rdf:about="http://purl.obolibrary.org/obo/GAZ_00251178">
        <obo:RO_0001025 rdf:resource="http://purl.obolibrary.org/obo/GAZ_00013505"/>
        <obo:IAO_0000115>A river.</obo:IAO_0000115>
        <oboInOwl:hasOBONamespace>GAZ</oboInOwl:hasOBONamespace>
        <oboInOwl:id>GAZ:00251178</oboInOwl:id>
        <rdfs:label>Hope River</rdfs:label>
    </owl:NamedIndividual>
    


    <!-- http://purl.obolibrary.org/obo/GAZ_00251179 -->

    <owl:NamedIndividual rdf:about="http://purl.obolibrary.org/obo/GAZ_00251179">
        <obo:RO_0001025 rdf:resource="http://purl.obolibrary.org/obo/GAZ_00013505"/>
        <obo:IAO_0000115>A river.</obo:IAO_0000115>
        <oboInOwl:hasOBONamespace>GAZ</oboInOwl:hasOBONamespace>
        <oboInOwl:id>GAZ:00251179</oboInOwl:id>
        <rdfs:label>Cane River</rdfs:label>
    </owl:NamedIndividual>
    


    <!-- http://purl.obolibrary.org/obo/GAZ_00251180 -->

    <owl:NamedIndividual rdf:about="http://purl.obolibrary.org/obo/GAZ_00251180">
        <obo:RO_0001025 rdf:resource="http://purl.obolibrary.org/obo/GAZ_00013513"/>
        <obo:IAO_0000115>A river.</obo:IAO_0000115>
        <oboInOwl:hasOBONamespace>GAZ</oboInOwl:hasOBONamespace>
        <oboInOwl:id>GAZ:00251180</oboInOwl:id>
        <rdfs:label>Yallahs River</rdfs:label>
    </owl:NamedIndividual>
    


    <!-- http://purl.obolibrary.org/obo/GAZ_00251181 -->

    <owl:NamedIndividual rdf:about="http://purl.obolibrary.org/obo/GAZ_00251181">
        <obo:RO_0001025 rdf:resource="http://purl.obolibrary.org/obo/GAZ_00013513"/>
        <obo:IAO_0000115>A river.</obo:IAO_0000115>
        <oboInOwl:hasOBONamespace>GAZ</oboInOwl:hasOBONamespace>
        <oboInOwl:id>GAZ:00251181</oboInOwl:id>
        <rdfs:label>Morant River</rdfs:label>
    </owl:NamedIndividual>
    


    <!-- http://purl.obolibrary.org/obo/GAZ_00251185 -->

    <owl:NamedIndividual rdf:about="http://purl.obolibrary.org/obo/GAZ_00251185">
        <obo:RO_0001025 rdf:resource="http://purl.obolibrary.org/obo/GAZ_00010070"/>
        <obo:IAO_0000115>A river.</obo:IAO_0000115>
        <oboInOwl:hasOBONamespace>GAZ</oboInOwl:hasOBONamespace>
        <oboInOwl:id>GAZ:00251185</oboInOwl:id>
        <rdfs:label>Lucea West River</rdfs:label>
    </owl:NamedIndividual>
    


    <!-- http://purl.obolibrary.org/obo/GAZ_00251186 -->

    <owl:NamedIndividual rdf:about="http://purl.obolibrary.org/obo/GAZ_00251186">
        <obo:RO_0001025 rdf:resource="http://purl.obolibrary.org/obo/GAZ_00010070"/>
        <obo:IAO_0000115>A river.</obo:IAO_0000115>
        <oboInOwl:hasOBONamespace>GAZ</oboInOwl:hasOBONamespace>
        <oboInOwl:id>GAZ:00251186</oboInOwl:id>
        <rdfs:label>Lucea East River</rdfs:label>
    </owl:NamedIndividual>
    


    <!-- http://purl.obolibrary.org/obo/GAZ_00251187 -->

    <owl:NamedIndividual rdf:about="http://purl.obolibrary.org/obo/GAZ_00251187">
        <obo:RO_0001025 rdf:resource="http://purl.obolibrary.org/obo/GAZ_00010070"/>
        <obo:IAO_0000115>A river.</obo:IAO_0000115>
        <oboInOwl:hasOBONamespace>GAZ</oboInOwl:hasOBONamespace>
        <oboInOwl:id>GAZ:00251187</oboInOwl:id>
        <rdfs:label>Flint River</rdfs:label>
    </owl:NamedIndividual>
    


    <!-- http://purl.obolibrary.org/obo/GAZ_00251188 -->

    <owl:NamedIndividual rdf:about="http://purl.obolibrary.org/obo/GAZ_00251188">
        <obo:RO_0001025 rdf:resource="http://purl.obolibrary.org/obo/GAZ_00013515"/>
        <obo:IAO_0000115>A river.</obo:IAO_0000115>
        <oboInOwl:hasOBONamespace>GAZ</oboInOwl:hasOBONamespace>
        <oboInOwl:id>GAZ:00251188</oboInOwl:id>
        <rdfs:label>Flint River</rdfs:label>
    </owl:NamedIndividual>
    


    <!-- http://purl.obolibrary.org/obo/GAZ_00251189 -->

    <owl:NamedIndividual rdf:about="http://purl.obolibrary.org/obo/GAZ_00251189">
        <obo:RO_0001025 rdf:resource="http://purl.obolibrary.org/obo/GAZ_00013515"/>
        <obo:IAO_0000115>A river.</obo:IAO_0000115>
        <oboInOwl:hasOBONamespace>GAZ</oboInOwl:hasOBONamespace>
        <oboInOwl:id>GAZ:00251189</oboInOwl:id>
        <rdfs:label>Wag Water River</rdfs:label>
    </owl:NamedIndividual>
    


    <!-- http://purl.obolibrary.org/obo/GAZ_00251190 -->

    <owl:NamedIndividual rdf:about="http://purl.obolibrary.org/obo/GAZ_00251190">
        <obo:RO_0001025 rdf:resource="http://purl.obolibrary.org/obo/GAZ_00013510"/>
        <obo:IAO_0000115>A river.</obo:IAO_0000115>
        <oboInOwl:hasOBONamespace>GAZ</oboInOwl:hasOBONamespace>
        <oboInOwl:id>GAZ:00251190</oboInOwl:id>
        <rdfs:label>Montego River</rdfs:label>
    </owl:NamedIndividual>
    


    <!-- http://purl.obolibrary.org/obo/GAZ_00251191 -->

    <owl:NamedIndividual rdf:about="http://purl.obolibrary.org/obo/GAZ_00251191">
        <obo:RO_0001025 rdf:resource="http://purl.obolibrary.org/obo/GAZ_00013514"/>
        <obo:IAO_0000115>A river.</obo:IAO_0000115>
        <oboInOwl:hasOBONamespace>GAZ</oboInOwl:hasOBONamespace>
        <oboInOwl:id>GAZ:00251191</oboInOwl:id>
        <rdfs:label>Martha Brae River</rdfs:label>
    </owl:NamedIndividual>
    


    <!-- http://purl.obolibrary.org/obo/GAZ_00251192 -->

    <owl:NamedIndividual rdf:about="http://purl.obolibrary.org/obo/GAZ_00251192">
        <obo:RO_0001025 rdf:resource="http://purl.obolibrary.org/obo/GAZ_00013514"/>
        <obo:IAO_0000115>A river.</obo:IAO_0000115>
        <oboInOwl:hasOBONamespace>GAZ</oboInOwl:hasOBONamespace>
        <oboInOwl:id>GAZ:00251192</oboInOwl:id>
        <rdfs:label>Rio Bueno</rdfs:label>
    </owl:NamedIndividual>
    


    <!-- http://purl.obolibrary.org/obo/GAZ_00251194 -->

    <owl:NamedIndividual rdf:about="http://purl.obolibrary.org/obo/GAZ_00251194">
        <obo:RO_0001025 rdf:resource="http://purl.obolibrary.org/obo/GAZ_00013515"/>
        <obo:IAO_0000115>A river.</obo:IAO_0000115>
        <oboInOwl:hasOBONamespace>GAZ</oboInOwl:hasOBONamespace>
        <oboInOwl:id>GAZ:00251194</oboInOwl:id>
        <rdfs:label>Rio Nuevo</rdfs:label>
    </owl:NamedIndividual>
    


    <!-- http://purl.obolibrary.org/obo/GAZ_00251195 -->

    <owl:NamedIndividual rdf:about="http://purl.obolibrary.org/obo/GAZ_00251195">
        <obo:RO_0001025 rdf:resource="http://purl.obolibrary.org/obo/GAZ_00013515"/>
        <obo:IAO_0000115>A river.</obo:IAO_0000115>
        <oboInOwl:hasOBONamespace>GAZ</oboInOwl:hasOBONamespace>
        <oboInOwl:id>GAZ:00251195</oboInOwl:id>
        <rdfs:label>Oracabessa River</rdfs:label>
    </owl:NamedIndividual>
    


    <!-- http://purl.obolibrary.org/obo/GAZ_00251198 -->

    <owl:NamedIndividual rdf:about="http://purl.obolibrary.org/obo/GAZ_00251198">
        <obo:RO_0001025 rdf:resource="http://purl.obolibrary.org/obo/GAZ_00004339"/>
        <obo:IAO_0000115>A river.</obo:IAO_0000115>
        <oboInOwl:hasOBONamespace>GAZ</oboInOwl:hasOBONamespace>
        <oboInOwl:id>GAZ:00251198</oboInOwl:id>
        <rdfs:label>Buff Bay River</rdfs:label>
    </owl:NamedIndividual>
    


    <!-- http://purl.obolibrary.org/obo/GAZ_00251199 -->

    <owl:NamedIndividual rdf:about="http://purl.obolibrary.org/obo/GAZ_00251199">
        <obo:RO_0001025 rdf:resource="http://purl.obolibrary.org/obo/GAZ_00013515"/>
        <obo:IAO_0000115>A river in Saint Mary, Jamaica. It reaches the sea in the parish capital of Port Maria.</obo:IAO_0000115>
        <oboInOwl:hasOBONamespace>GAZ</oboInOwl:hasOBONamespace>
        <oboInOwl:id>GAZ:00251199</oboInOwl:id>
        <rdfs:label>Otram River</rdfs:label>
    </owl:NamedIndividual>
    


    <!-- http://purl.obolibrary.org/obo/GAZ_00251200 -->

    <owl:NamedIndividual rdf:about="http://purl.obolibrary.org/obo/GAZ_00251200">
        <obo:RO_0001025 rdf:resource="http://purl.obolibrary.org/obo/GAZ_00004339"/>
        <obo:IAO_0000115>A river.</obo:IAO_0000115>
        <oboInOwl:hasOBONamespace>GAZ</oboInOwl:hasOBONamespace>
        <oboInOwl:id>GAZ:00251200</oboInOwl:id>
        <rdfs:label>Spanish River</rdfs:label>
    </owl:NamedIndividual>
    


    <!-- http://purl.obolibrary.org/obo/GAZ_00251201 -->

    <owl:NamedIndividual rdf:about="http://purl.obolibrary.org/obo/GAZ_00251201">
        <obo:RO_0001025 rdf:resource="http://purl.obolibrary.org/obo/GAZ_00004339"/>
        <obo:IAO_0000115>A river.</obo:IAO_0000115>
        <oboInOwl:hasOBONamespace>GAZ</oboInOwl:hasOBONamespace>
        <oboInOwl:id>GAZ:00251201</oboInOwl:id>
        <rdfs:label>Swift River</rdfs:label>
    </owl:NamedIndividual>
    


    <!-- http://purl.obolibrary.org/obo/GAZ_00251202 -->

    <owl:NamedIndividual rdf:about="http://purl.obolibrary.org/obo/GAZ_00251202">
        <obo:RO_0001025 rdf:resource="http://purl.obolibrary.org/obo/GAZ_00013513"/>
        <obo:IAO_0000115>A river.</obo:IAO_0000115>
        <oboInOwl:hasOBONamespace>GAZ</oboInOwl:hasOBONamespace>
        <oboInOwl:id>GAZ:00251202</oboInOwl:id>
        <rdfs:label>Plantain Garden River</rdfs:label>
    </owl:NamedIndividual>
    


    <!-- http://purl.obolibrary.org/obo/GAZ_00251203 -->

    <owl:NamedIndividual rdf:about="http://purl.obolibrary.org/obo/GAZ_00251203">
        <obo:RO_0001025 rdf:resource="http://purl.obolibrary.org/obo/GAZ_00004339"/>
        <obo:IAO_0000115>A river.</obo:IAO_0000115>
        <oboInOwl:hasOBONamespace>GAZ</oboInOwl:hasOBONamespace>
        <oboInOwl:id>GAZ:00251203</oboInOwl:id>
        <rdfs:label>Rio Grande</rdfs:label>
    </owl:NamedIndividual>
    


    <!-- 
    ///////////////////////////////////////////////////////////////////////////////////////
    //
    // Annotations
    //
    ///////////////////////////////////////////////////////////////////////////////////////
     -->

    <rdf:Description rdf:about="http://purl.obolibrary.org/obo/GAZ_00004312">
        <oboInOwl:hasOBONamespace>GAZ</oboInOwl:hasOBONamespace>
        <rdfs:label>County (Jamaica)</rdfs:label>
        <oboInOwl:id>GAZ:00004312</oboInOwl:id>
    </rdf:Description>
    <rdf:Description rdf:about="http://purl.obolibrary.org/obo/GAZ_00008622">
        <oboInOwl:id>GAZ:00008622</oboInOwl:id>
        <rdfs:label>populated place, Jamaica</rdfs:label>
        <oboInOwl:hasOBONamespace>GAZ</oboInOwl:hasOBONamespace>
    </rdf:Description>
    <rdf:Description rdf:about="http://purl.obolibrary.org/obo/GAZ_00010072">
        <oboInOwl:hasOBONamespace>GAZ</oboInOwl:hasOBONamespace>
        <rdfs:label>Negril</rdfs:label>
        <obo:IAO_0000115>A large beach resort located across parts of two Jamaican parishes, Westmoreland and Hanover.</obo:IAO_0000115>
        <oboInOwl:id>GAZ:00010072</oboInOwl:id>
    </rdf:Description>
    <rdf:Description rdf:about="http://purl.obolibrary.org/obo/GAZ_00013516">
        <rdfs:label>County of Cornwall</rdfs:label>
        <oboInOwl:hasOBONamespace>GAZ</oboInOwl:hasOBONamespace>
        <oboInOwl:id>GAZ:00013516</oboInOwl:id>
        <obo:IAO_0000115>The westernmost of the three counties into which Jamaica is divided. It includes Montego Bay, the second city.</obo:IAO_0000115>
    </rdf:Description>
    <rdf:Description rdf:about="http://purl.obolibrary.org/obo/GAZ_00013517">
        <obo:IAO_0000115>The easternmost and the smallest by area of the three counties into which Jamaica is divided.</obo:IAO_0000115>
        <oboInOwl:id>GAZ:00013517</oboInOwl:id>
        <oboInOwl:hasOBONamespace>GAZ</oboInOwl:hasOBONamespace>
        <rdfs:label>County of Surrey</rdfs:label>
    </rdf:Description>
    <rdf:Description rdf:about="http://purl.obolibrary.org/obo/GAZ_00013518">
        <obo:IAO_0000115>The central of the three counties into which Jamaica is divided.</obo:IAO_0000115>
        <oboInOwl:id>GAZ:00013518</oboInOwl:id>
        <oboInOwl:hasOBONamespace>GAZ</oboInOwl:hasOBONamespace>
        <rdfs:label>County of Middlesex</rdfs:label>
    </rdf:Description>
</rdf:RDF>



<!-- Generated by the OWL API (version 4.5.6) https://github.com/owlcs/owlapi -->

