<?xml version="1.0"?>
<rdf:RDF xmlns="http://purl.obolibrary.org/obo/gaz/subsets/countries/Jordan.owl#"
     xml:base="http://purl.obolibrary.org/obo/gaz/subsets/countries/Jordan.owl"
     xmlns:obo="http://purl.obolibrary.org/obo/"
     xmlns:owl="http://www.w3.org/2002/07/owl#"
     xmlns:rdf="http://www.w3.org/1999/02/22-rdf-syntax-ns#"
     xmlns:xml="http://www.w3.org/XML/1998/namespace"
     xmlns:xsd="http://www.w3.org/2001/XMLSchema#"
     xmlns:rdfs="http://www.w3.org/2000/01/rdf-schema#"
     xmlns:oboInOwl="http://www.geneontology.org/formats/oboInOwl#">
    <owl:Ontology rdf:about="http://purl.obolibrary.org/obo/gaz/subsets/countries/Jordan.owl">
        <owl:imports rdf:resource="http://purl.obolibrary.org/obo/gaz/imports/envo_import.owl"/>
        <owl:imports rdf:resource="http://purl.obolibrary.org/obo/gaz/imports/ro_import.owl"/>
    </owl:Ontology>
    


    <!-- 
    ///////////////////////////////////////////////////////////////////////////////////////
    //
    // Annotation properties
    //
    ///////////////////////////////////////////////////////////////////////////////////////
     -->

    


    <!-- http://purl.obolibrary.org/obo/IAO_0000115 -->

    <owl:AnnotationProperty rdf:about="http://purl.obolibrary.org/obo/IAO_0000115"/>
    


    <!-- http://www.geneontology.org/formats/oboInOwl#hasOBONamespace -->

    <owl:AnnotationProperty rdf:about="http://www.geneontology.org/formats/oboInOwl#hasOBONamespace"/>
    


    <!-- http://www.geneontology.org/formats/oboInOwl#id -->

    <owl:AnnotationProperty rdf:about="http://www.geneontology.org/formats/oboInOwl#id"/>
    


    <!-- 
    ///////////////////////////////////////////////////////////////////////////////////////
    //
    // Object Properties
    //
    ///////////////////////////////////////////////////////////////////////////////////////
     -->

    


    <!-- http://purl.obolibrary.org/obo/RO_0001025 -->

    <owl:ObjectProperty rdf:about="http://purl.obolibrary.org/obo/RO_0001025"/>
    


    <!-- 
    ///////////////////////////////////////////////////////////////////////////////////////
    //
    // Classes
    //
    ///////////////////////////////////////////////////////////////////////////////////////
     -->

    


    <!-- http://purl.obolibrary.org/obo/ENVO_00000009 -->

    <owl:Class rdf:about="http://purl.obolibrary.org/obo/ENVO_00000009"/>
    


    <!-- http://purl.obolibrary.org/obo/ENVO_00000032 -->

    <owl:Class rdf:about="http://purl.obolibrary.org/obo/ENVO_00000032"/>
    


    <!-- http://purl.obolibrary.org/obo/ENVO_00000196 -->

    <owl:Class rdf:about="http://purl.obolibrary.org/obo/ENVO_00000196"/>
    


    <!-- http://purl.obolibrary.org/obo/ENVO_00000856 -->

    <owl:Class rdf:about="http://purl.obolibrary.org/obo/ENVO_00000856"/>
    


    <!-- http://purl.obolibrary.org/obo/GAZ_00009510 -->

    <owl:Class rdf:about="http://purl.obolibrary.org/obo/GAZ_00009510"/>
    


    <!-- http://purl.obolibrary.org/obo/GAZ_02000738 -->

    <owl:Class rdf:about="http://purl.obolibrary.org/obo/GAZ_02000738">
        <rdfs:subClassOf rdf:resource="http://purl.obolibrary.org/obo/GAZ_00009510"/>
    </owl:Class>
    


    <!-- http://purl.obolibrary.org/obo/GAZ_02000739 -->

    <owl:Class rdf:about="http://purl.obolibrary.org/obo/GAZ_02000739">
        <rdfs:subClassOf rdf:resource="http://purl.obolibrary.org/obo/GAZ_00009510"/>
    </owl:Class>
    


    <!-- http://purl.obolibrary.org/obo/GAZ_02000740 -->

    <owl:Class rdf:about="http://purl.obolibrary.org/obo/GAZ_02000740">
        <rdfs:subClassOf rdf:resource="http://purl.obolibrary.org/obo/GAZ_00009510"/>
    </owl:Class>
    


    <!-- http://purl.obolibrary.org/obo/GAZ_02000741 -->

    <owl:Class rdf:about="http://purl.obolibrary.org/obo/GAZ_02000741">
        <rdfs:subClassOf rdf:resource="http://purl.obolibrary.org/obo/GAZ_00009510"/>
    </owl:Class>
    


    <!-- http://purl.obolibrary.org/obo/GAZ_02000742 -->

    <owl:Class rdf:about="http://purl.obolibrary.org/obo/GAZ_02000742">
        <rdfs:subClassOf rdf:resource="http://purl.obolibrary.org/obo/GAZ_00009510"/>
    </owl:Class>
    


    <!-- http://purl.obolibrary.org/obo/GAZ_02000743 -->

    <owl:Class rdf:about="http://purl.obolibrary.org/obo/GAZ_02000743">
        <rdfs:subClassOf rdf:resource="http://purl.obolibrary.org/obo/GAZ_00009510"/>
    </owl:Class>
    


    <!-- http://purl.obolibrary.org/obo/GAZ_02000744 -->

    <owl:Class rdf:about="http://purl.obolibrary.org/obo/GAZ_02000744">
        <rdfs:subClassOf rdf:resource="http://purl.obolibrary.org/obo/GAZ_00009510"/>
    </owl:Class>
    


    <!-- http://purl.obolibrary.org/obo/GAZ_02000745 -->

    <owl:Class rdf:about="http://purl.obolibrary.org/obo/GAZ_02000745">
        <rdfs:subClassOf rdf:resource="http://purl.obolibrary.org/obo/GAZ_00009510"/>
    </owl:Class>
    


    <!-- http://purl.obolibrary.org/obo/GAZ_02000746 -->

    <owl:Class rdf:about="http://purl.obolibrary.org/obo/GAZ_02000746">
        <rdfs:subClassOf rdf:resource="http://purl.obolibrary.org/obo/GAZ_00009510"/>
    </owl:Class>
    


    <!-- http://purl.obolibrary.org/obo/GAZ_02000747 -->

    <owl:Class rdf:about="http://purl.obolibrary.org/obo/GAZ_02000747">
        <rdfs:subClassOf rdf:resource="http://purl.obolibrary.org/obo/GAZ_00009510"/>
    </owl:Class>
    


    <!-- http://purl.obolibrary.org/obo/GAZ_02000748 -->

    <owl:Class rdf:about="http://purl.obolibrary.org/obo/GAZ_02000748">
        <rdfs:subClassOf rdf:resource="http://purl.obolibrary.org/obo/GAZ_00009510"/>
    </owl:Class>
    


    <!-- http://purl.obolibrary.org/obo/GAZ_02000749 -->

    <owl:Class rdf:about="http://purl.obolibrary.org/obo/GAZ_02000749">
        <rdfs:subClassOf rdf:resource="http://purl.obolibrary.org/obo/GAZ_00009510"/>
    </owl:Class>
    


    <!-- 
    ///////////////////////////////////////////////////////////////////////////////////////
    //
    // Individuals
    //
    ///////////////////////////////////////////////////////////////////////////////////////
     -->

    


    <!-- http://purl.obolibrary.org/obo/GAZ_00002473 -->

    <owl:NamedIndividual rdf:about="http://purl.obolibrary.org/obo/GAZ_00002473">
        <rdf:type rdf:resource="http://purl.obolibrary.org/obo/ENVO_00000009"/>
        <obo:IAO_0000115>A country in Southwest Asia, bordered by Syria to the north, Iraq to the north-east, Israel and the West Bank to the west, and Saudi Arabia to the east and south. It shares the coastlines of the Dead Sea, and the Gulf of Aqaba with Israel, Saudi Arabia, and Egypt. Jordan is divided into 12 provinces called governorates. The Governorates are subdivided into approximately fifty-two nahias.</obo:IAO_0000115>
        <oboInOwl:hasOBONamespace>GAZ</oboInOwl:hasOBONamespace>
        <oboInOwl:id>GAZ:00002473</oboInOwl:id>
        <rdfs:label>Jordan</rdfs:label>
    </owl:NamedIndividual>
    


    <!-- http://purl.obolibrary.org/obo/GAZ_00002477 -->

    <owl:NamedIndividual rdf:about="http://purl.obolibrary.org/obo/GAZ_00002477">
        <obo:RO_0001025 rdf:resource="http://purl.obolibrary.org/obo/GAZ_00007520"/>
        <obo:IAO_0000115>A saline lake between the West Bank and Israel to the west, and Jordan to the east.</obo:IAO_0000115>
        <oboInOwl:hasOBONamespace>GAZ</oboInOwl:hasOBONamespace>
        <oboInOwl:id>GAZ:00002477</oboInOwl:id>
        <rdfs:label>Dead Sea</rdfs:label>
    </owl:NamedIndividual>
    


    <!-- http://purl.obolibrary.org/obo/GAZ_00007520 -->

    <owl:NamedIndividual rdf:about="http://purl.obolibrary.org/obo/GAZ_00007520">
        <obo:RO_0001025 rdf:resource="http://purl.obolibrary.org/obo/GAZ_00044915"/>
        <obo:IAO_0000115>A river in Southwest Asia flowing through the Great Rift Valley into the Dead Sea.</obo:IAO_0000115>
        <oboInOwl:hasOBONamespace>GAZ</oboInOwl:hasOBONamespace>
        <oboInOwl:id>GAZ:00007520</oboInOwl:id>
        <rdfs:label>River Jordan</rdfs:label>
    </owl:NamedIndividual>
    


    <!-- http://purl.obolibrary.org/obo/GAZ_00007862 -->

    <owl:NamedIndividual rdf:about="http://purl.obolibrary.org/obo/GAZ_00007862">
        <rdf:type rdf:resource="http://purl.obolibrary.org/obo/ENVO_00000032"/>
        <obo:IAO_0000115>A gulf situated northeastward and adjacent to the Red Sea, bounded by the coasts of Sinai Peninsula and Arabian Peninsula. Its southern limit with the Red Sea (in the Strait of T Degrees r Degrees n) is the following: A line joining Cape Al Qa Degrees bah (28 Degrees 01430 Seconds N - 34 Degrees 37 Minutes 15 Seconds E), in Saudi Arabia, southwestward to position 27 Degrees 58 Minutes 10 Seconds N - 34 Degrees 35 Minutes E) on the coast of T Degrees r Degrees n Island; thence from this position southward, through T Degrees r Degrees n Island, to its southwestern extremity (27 Degrees 54 Minutes 50 Seconds N - 34 Degrees 33 Minutes E); and thence from the southwestern extremity of T Degrees r Degrees n Island westward, along the parallel of 27 Degrees 54 Minutes 50 Seconds N, to the coast of Sinai Peninsula, in Egypt.</obo:IAO_0000115>
        <oboInOwl:hasOBONamespace>GAZ</oboInOwl:hasOBONamespace>
        <oboInOwl:id>GAZ:00007862</oboInOwl:id>
        <rdfs:label>Gulf of Aqaba</rdfs:label>
    </owl:NamedIndividual>
    


    <!-- http://purl.obolibrary.org/obo/GAZ_00008742 -->

    <owl:NamedIndividual rdf:about="http://purl.obolibrary.org/obo/GAZ_00008742">
        <obo:RO_0001025 rdf:resource="http://purl.obolibrary.org/obo/GAZ_00044915"/>
        <obo:IAO_0000115>A valley that lies within the northern part of the Syrian-African Rift Valley at an elevation of about 70 m above sea level. On both sides of the valley are steep slopes -- the Golan Heights to the east and the Upper Galilee mountains to the west, rise to 400 to 900 m above sea level. Basaltic hills of about 200 m above sea level along the southern side of the valley intercept the Jordan River, and are commonly referred to as the basalt &quot;plug&quot; (actually a temporary geologic base level), as they restrict water drainage downstream into the Sea of Galilee (Lake Kinneret). The Hula Valley covers an area of 177 km2 (25 km by 6-8 km.</obo:IAO_0000115>
        <oboInOwl:hasOBONamespace>GAZ</oboInOwl:hasOBONamespace>
        <oboInOwl:id>GAZ:00008742</oboInOwl:id>
        <rdfs:label>Hulah Valley</rdfs:label>
    </owl:NamedIndividual>
    


    <!-- http://purl.obolibrary.org/obo/GAZ_00008743 -->

    <owl:NamedIndividual rdf:about="http://purl.obolibrary.org/obo/GAZ_00008743">
        <obo:RO_0001025 rdf:resource="http://purl.obolibrary.org/obo/GAZ_00193886"/>
        <obo:IAO_0000115>A wetland.</obo:IAO_0000115>
        <oboInOwl:hasOBONamespace>GAZ</oboInOwl:hasOBONamespace>
        <oboInOwl:id>GAZ:00008743</oboInOwl:id>
        <rdfs:label>Hulah Swamp</rdfs:label>
    </owl:NamedIndividual>
    


    <!-- http://purl.obolibrary.org/obo/GAZ_00009510 -->

    <owl:NamedIndividual rdf:about="http://purl.obolibrary.org/obo/GAZ_00009510">
        <obo:RO_0001025 rdf:resource="http://purl.obolibrary.org/obo/GAZ_00002473"/>
    </owl:NamedIndividual>
    


    <!-- http://purl.obolibrary.org/obo/GAZ_00010533 -->

    <owl:NamedIndividual rdf:about="http://purl.obolibrary.org/obo/GAZ_00010533">
        <obo:RO_0001025 rdf:resource="http://purl.obolibrary.org/obo/GAZ_00044915"/>
        <obo:IAO_0000115>A large fertile plain and inland valley in the south of the Lower Galilee region of Israel. It is bordered to the south by the Samaria highlands and Mount Gilboa, to the north by the Lower Galilee, to the west by the Mount Carmel range, and to the east by the Jordan Valley.</obo:IAO_0000115>
        <oboInOwl:hasOBONamespace>GAZ</oboInOwl:hasOBONamespace>
        <oboInOwl:id>GAZ:00010533</oboInOwl:id>
        <rdfs:label>Jezreel Valley</rdfs:label>
    </owl:NamedIndividual>
    


    <!-- http://purl.obolibrary.org/obo/GAZ_00014012 -->

    <owl:NamedIndividual rdf:about="http://purl.obolibrary.org/obo/GAZ_00014012">
        <obo:IAO_0000115>A volcanic field that lies in the Haurun-Druze Plateau in SW Syria near the border with Jordan. The most prominent feature of this volcanic field is 1800 m high Jabal ad Druze (also known variously as Djebel Al-Arab, Jabal ed Duruz, Jabal al Druz, Jebel Duraz, Djebel ed Drouz). The alkaline volcanic field consists of a group of 118 basaltic volcanoes active from the lower-Pleistocene to the Holocene. The large SW Plateau depression is filled by basaltic lava flows from volcanoes aligned in a NW-SE direction. This volcanic field lies within the northern part of the massive alkaline Harrat Ash Shaam volcanic field that extends from southern Syria through NW Jordan to Saudi Arabia.</obo:IAO_0000115>
        <oboInOwl:hasOBONamespace>GAZ</oboInOwl:hasOBONamespace>
        <oboInOwl:id>GAZ:00014012</oboInOwl:id>
        <rdfs:label>Jabal ad-Duruz Volcanic Field</rdfs:label>
    </owl:NamedIndividual>
    


    <!-- http://purl.obolibrary.org/obo/GAZ_00030846 -->

    <owl:NamedIndividual rdf:about="http://purl.obolibrary.org/obo/GAZ_00030846">
        <obo:RO_0001025 rdf:resource="http://purl.obolibrary.org/obo/GAZ_02000746"/>
        <oboInOwl:hasOBONamespace>GAZ</oboInOwl:hasOBONamespace>
        <oboInOwl:id>GAZ:00030846</oboInOwl:id>
        <rdfs:label>Kofranjah Subdistrict</rdfs:label>
    </owl:NamedIndividual>
    


    <!-- http://purl.obolibrary.org/obo/GAZ_00030847 -->

    <owl:NamedIndividual rdf:about="http://purl.obolibrary.org/obo/GAZ_00030847">
        <obo:RO_0001025 rdf:resource="http://purl.obolibrary.org/obo/GAZ_02000746"/>
        <oboInOwl:hasOBONamespace>GAZ</oboInOwl:hasOBONamespace>
        <oboInOwl:id>GAZ:00030847</oboInOwl:id>
        <rdfs:label>Ajlun Subdistrict</rdfs:label>
    </owl:NamedIndividual>
    


    <!-- http://purl.obolibrary.org/obo/GAZ_00030848 -->

    <owl:NamedIndividual rdf:about="http://purl.obolibrary.org/obo/GAZ_00030848">
        <obo:RO_0001025 rdf:resource="http://purl.obolibrary.org/obo/GAZ_02000747"/>
        <oboInOwl:hasOBONamespace>GAZ</oboInOwl:hasOBONamespace>
        <oboInOwl:id>GAZ:00030848</oboInOwl:id>
        <rdfs:label>Na&apos;oor Subdistrict</rdfs:label>
    </owl:NamedIndividual>
    


    <!-- http://purl.obolibrary.org/obo/GAZ_00030849 -->

    <owl:NamedIndividual rdf:about="http://purl.obolibrary.org/obo/GAZ_00030849">
        <obo:RO_0001025 rdf:resource="http://purl.obolibrary.org/obo/GAZ_02000747"/>
        <oboInOwl:hasOBONamespace>GAZ</oboInOwl:hasOBONamespace>
        <oboInOwl:id>GAZ:00030849</oboInOwl:id>
        <rdfs:label>Sahab Subdistrict</rdfs:label>
    </owl:NamedIndividual>
    


    <!-- http://purl.obolibrary.org/obo/GAZ_00030850 -->

    <owl:NamedIndividual rdf:about="http://purl.obolibrary.org/obo/GAZ_00030850">
        <obo:RO_0001025 rdf:resource="http://purl.obolibrary.org/obo/GAZ_02000747"/>
        <oboInOwl:hasOBONamespace>GAZ</oboInOwl:hasOBONamespace>
        <oboInOwl:id>GAZ:00030850</oboInOwl:id>
        <rdfs:label>Wadi al-Sayr Subdistrict</rdfs:label>
    </owl:NamedIndividual>
    


    <!-- http://purl.obolibrary.org/obo/GAZ_00030851 -->

    <owl:NamedIndividual rdf:about="http://purl.obolibrary.org/obo/GAZ_00030851">
        <obo:RO_0001025 rdf:resource="http://purl.obolibrary.org/obo/GAZ_02000747"/>
        <oboInOwl:hasOBONamespace>GAZ</oboInOwl:hasOBONamespace>
        <oboInOwl:id>GAZ:00030851</oboInOwl:id>
        <rdfs:label>Um al-Basatin Subdistrict</rdfs:label>
    </owl:NamedIndividual>
    


    <!-- http://purl.obolibrary.org/obo/GAZ_00030852 -->

    <owl:NamedIndividual rdf:about="http://purl.obolibrary.org/obo/GAZ_00030852">
        <obo:RO_0001025 rdf:resource="http://purl.obolibrary.org/obo/GAZ_02000747"/>
        <oboInOwl:hasOBONamespace>GAZ</oboInOwl:hasOBONamespace>
        <oboInOwl:id>GAZ:00030852</oboInOwl:id>
        <rdfs:label>Al-Mwwqqar Subdistrict</rdfs:label>
    </owl:NamedIndividual>
    


    <!-- http://purl.obolibrary.org/obo/GAZ_00030853 -->

    <owl:NamedIndividual rdf:about="http://purl.obolibrary.org/obo/GAZ_00030853">
        <obo:RO_0001025 rdf:resource="http://purl.obolibrary.org/obo/GAZ_02000747"/>
        <oboInOwl:hasOBONamespace>GAZ</oboInOwl:hasOBONamespace>
        <oboInOwl:id>GAZ:00030853</oboInOwl:id>
        <rdfs:label>Amman Subdistrict</rdfs:label>
    </owl:NamedIndividual>
    


    <!-- http://purl.obolibrary.org/obo/GAZ_00030854 -->

    <owl:NamedIndividual rdf:about="http://purl.obolibrary.org/obo/GAZ_00030854">
        <obo:RO_0001025 rdf:resource="http://purl.obolibrary.org/obo/GAZ_02000747"/>
        <oboInOwl:hasOBONamespace>GAZ</oboInOwl:hasOBONamespace>
        <oboInOwl:id>GAZ:00030854</oboInOwl:id>
        <rdfs:label>Al-Jiza Subdistrict</rdfs:label>
    </owl:NamedIndividual>
    


    <!-- http://purl.obolibrary.org/obo/GAZ_00030855 -->

    <owl:NamedIndividual rdf:about="http://purl.obolibrary.org/obo/GAZ_00030855">
        <obo:RO_0001025 rdf:resource="http://purl.obolibrary.org/obo/GAZ_02000745"/>
        <oboInOwl:hasOBONamespace>GAZ</oboInOwl:hasOBONamespace>
        <oboInOwl:id>GAZ:00030855</oboInOwl:id>
        <rdfs:label>Al-Quwayra Subdistrict</rdfs:label>
    </owl:NamedIndividual>
    


    <!-- http://purl.obolibrary.org/obo/GAZ_00030856 -->

    <owl:NamedIndividual rdf:about="http://purl.obolibrary.org/obo/GAZ_00030856">
        <obo:RO_0001025 rdf:resource="http://purl.obolibrary.org/obo/GAZ_02000745"/>
        <oboInOwl:hasOBONamespace>GAZ</oboInOwl:hasOBONamespace>
        <oboInOwl:id>GAZ:00030856</oboInOwl:id>
        <rdfs:label>Al-Aqaba Subdistrict</rdfs:label>
    </owl:NamedIndividual>
    


    <!-- http://purl.obolibrary.org/obo/GAZ_00030857 -->

    <owl:NamedIndividual rdf:about="http://purl.obolibrary.org/obo/GAZ_00030857">
        <obo:RO_0001025 rdf:resource="http://purl.obolibrary.org/obo/GAZ_02000745"/>
        <oboInOwl:hasOBONamespace>GAZ</oboInOwl:hasOBONamespace>
        <oboInOwl:id>GAZ:00030857</oboInOwl:id>
        <rdfs:label>Wadi Araba Subdistrict</rdfs:label>
    </owl:NamedIndividual>
    


    <!-- http://purl.obolibrary.org/obo/GAZ_00030858 -->

    <owl:NamedIndividual rdf:about="http://purl.obolibrary.org/obo/GAZ_00030858">
        <obo:RO_0001025 rdf:resource="http://purl.obolibrary.org/obo/GAZ_02000742"/>
        <oboInOwl:hasOBONamespace>GAZ</oboInOwl:hasOBONamespace>
        <oboInOwl:id>GAZ:00030858</oboInOwl:id>
        <rdfs:label>Ardhah Subdistrict</rdfs:label>
    </owl:NamedIndividual>
    


    <!-- http://purl.obolibrary.org/obo/GAZ_00030859 -->

    <owl:NamedIndividual rdf:about="http://purl.obolibrary.org/obo/GAZ_00030859">
        <obo:RO_0001025 rdf:resource="http://purl.obolibrary.org/obo/GAZ_02000742"/>
        <oboInOwl:hasOBONamespace>GAZ</oboInOwl:hasOBONamespace>
        <oboInOwl:id>GAZ:00030859</oboInOwl:id>
        <rdfs:label>Al-Balqa Subdistrict</rdfs:label>
    </owl:NamedIndividual>
    


    <!-- http://purl.obolibrary.org/obo/GAZ_00030860 -->

    <owl:NamedIndividual rdf:about="http://purl.obolibrary.org/obo/GAZ_00030860">
        <obo:RO_0001025 rdf:resource="http://purl.obolibrary.org/obo/GAZ_02000742"/>
        <oboInOwl:hasOBONamespace>GAZ</oboInOwl:hasOBONamespace>
        <oboInOwl:id>GAZ:00030860</oboInOwl:id>
        <rdfs:label>Shuna al-Janibiyya Subdistrict</rdfs:label>
    </owl:NamedIndividual>
    


    <!-- http://purl.obolibrary.org/obo/GAZ_00030861 -->

    <owl:NamedIndividual rdf:about="http://purl.obolibrary.org/obo/GAZ_00030861">
        <obo:RO_0001025 rdf:resource="http://purl.obolibrary.org/obo/GAZ_02000742"/>
        <oboInOwl:hasOBONamespace>GAZ</oboInOwl:hasOBONamespace>
        <oboInOwl:id>GAZ:00030861</oboInOwl:id>
        <rdfs:label>Dair Alla Subdistrict</rdfs:label>
    </owl:NamedIndividual>
    


    <!-- http://purl.obolibrary.org/obo/GAZ_00030862 -->

    <owl:NamedIndividual rdf:about="http://purl.obolibrary.org/obo/GAZ_00030862">
        <obo:RO_0001025 rdf:resource="http://purl.obolibrary.org/obo/GAZ_02000742"/>
        <oboInOwl:hasOBONamespace>GAZ</oboInOwl:hasOBONamespace>
        <oboInOwl:id>GAZ:00030862</oboInOwl:id>
        <rdfs:label>As-Salt Subdistrict</rdfs:label>
    </owl:NamedIndividual>
    


    <!-- http://purl.obolibrary.org/obo/GAZ_00030863 -->

    <owl:NamedIndividual rdf:about="http://purl.obolibrary.org/obo/GAZ_00030863">
        <obo:RO_0001025 rdf:resource="http://purl.obolibrary.org/obo/GAZ_02000743"/>
        <oboInOwl:hasOBONamespace>GAZ</oboInOwl:hasOBONamespace>
        <oboInOwl:id>GAZ:00030863</oboInOwl:id>
        <rdfs:label>Mazar Shamaliyyeh Subdistrict</rdfs:label>
    </owl:NamedIndividual>
    


    <!-- http://purl.obolibrary.org/obo/GAZ_00030864 -->

    <owl:NamedIndividual rdf:about="http://purl.obolibrary.org/obo/GAZ_00030864">
        <obo:RO_0001025 rdf:resource="http://purl.obolibrary.org/obo/GAZ_02000743"/>
        <oboInOwl:hasOBONamespace>GAZ</oboInOwl:hasOBONamespace>
        <oboInOwl:id>GAZ:00030864</oboInOwl:id>
        <rdfs:label>Tayybeh Subdistrict</rdfs:label>
    </owl:NamedIndividual>
    


    <!-- http://purl.obolibrary.org/obo/GAZ_00030865 -->

    <owl:NamedIndividual rdf:about="http://purl.obolibrary.org/obo/GAZ_00030865">
        <obo:RO_0001025 rdf:resource="http://purl.obolibrary.org/obo/GAZ_02000743"/>
        <oboInOwl:hasOBONamespace>GAZ</oboInOwl:hasOBONamespace>
        <oboInOwl:id>GAZ:00030865</oboInOwl:id>
        <rdfs:label>Wastiyyeh Subdistrict</rdfs:label>
    </owl:NamedIndividual>
    


    <!-- http://purl.obolibrary.org/obo/GAZ_00030866 -->

    <owl:NamedIndividual rdf:about="http://purl.obolibrary.org/obo/GAZ_00030866">
        <obo:RO_0001025 rdf:resource="http://purl.obolibrary.org/obo/GAZ_02000743"/>
        <oboInOwl:hasOBONamespace>GAZ</oboInOwl:hasOBONamespace>
        <oboInOwl:id>GAZ:00030866</oboInOwl:id>
        <rdfs:label>Irbid Subdistrict</rdfs:label>
    </owl:NamedIndividual>
    


    <!-- http://purl.obolibrary.org/obo/GAZ_00030867 -->

    <owl:NamedIndividual rdf:about="http://purl.obolibrary.org/obo/GAZ_00030867">
        <obo:RO_0001025 rdf:resource="http://purl.obolibrary.org/obo/GAZ_02000743"/>
        <oboInOwl:hasOBONamespace>GAZ</oboInOwl:hasOBONamespace>
        <oboInOwl:id>GAZ:00030867</oboInOwl:id>
        <rdfs:label>Al-Aghwar Shamaliyyeh Subdistrict</rdfs:label>
    </owl:NamedIndividual>
    


    <!-- http://purl.obolibrary.org/obo/GAZ_00030868 -->

    <owl:NamedIndividual rdf:about="http://purl.obolibrary.org/obo/GAZ_00030868">
        <obo:RO_0001025 rdf:resource="http://purl.obolibrary.org/obo/GAZ_02000743"/>
        <oboInOwl:hasOBONamespace>GAZ</oboInOwl:hasOBONamespace>
        <oboInOwl:id>GAZ:00030868</oboInOwl:id>
        <rdfs:label>Ar Ramtha Subdistrict</rdfs:label>
    </owl:NamedIndividual>
    


    <!-- http://purl.obolibrary.org/obo/GAZ_00030869 -->

    <owl:NamedIndividual rdf:about="http://purl.obolibrary.org/obo/GAZ_00030869">
        <obo:RO_0001025 rdf:resource="http://purl.obolibrary.org/obo/GAZ_02000743"/>
        <oboInOwl:hasOBONamespace>GAZ</oboInOwl:hasOBONamespace>
        <oboInOwl:id>GAZ:00030869</oboInOwl:id>
        <rdfs:label>Kora Subdistrict</rdfs:label>
    </owl:NamedIndividual>
    


    <!-- http://purl.obolibrary.org/obo/GAZ_00030870 -->

    <owl:NamedIndividual rdf:about="http://purl.obolibrary.org/obo/GAZ_00030870">
        <obo:RO_0001025 rdf:resource="http://purl.obolibrary.org/obo/GAZ_02000743"/>
        <oboInOwl:hasOBONamespace>GAZ</oboInOwl:hasOBONamespace>
        <oboInOwl:id>GAZ:00030870</oboInOwl:id>
        <rdfs:label>Bani Knana Subdistrict</rdfs:label>
    </owl:NamedIndividual>
    


    <!-- http://purl.obolibrary.org/obo/GAZ_00030871 -->

    <owl:NamedIndividual rdf:about="http://purl.obolibrary.org/obo/GAZ_00030871">
        <obo:RO_0001025 rdf:resource="http://purl.obolibrary.org/obo/GAZ_02000743"/>
        <oboInOwl:hasOBONamespace>GAZ</oboInOwl:hasOBONamespace>
        <oboInOwl:id>GAZ:00030871</oboInOwl:id>
        <rdfs:label>Hariema Subdistrict</rdfs:label>
    </owl:NamedIndividual>
    


    <!-- http://purl.obolibrary.org/obo/GAZ_00030872 -->

    <owl:NamedIndividual rdf:about="http://purl.obolibrary.org/obo/GAZ_00030872">
        <obo:RO_0001025 rdf:resource="http://purl.obolibrary.org/obo/GAZ_02000738"/>
        <oboInOwl:hasOBONamespace>GAZ</oboInOwl:hasOBONamespace>
        <oboInOwl:id>GAZ:00030872</oboInOwl:id>
        <rdfs:label>Jerash Subdistrict</rdfs:label>
    </owl:NamedIndividual>
    


    <!-- http://purl.obolibrary.org/obo/GAZ_00030873 -->

    <owl:NamedIndividual rdf:about="http://purl.obolibrary.org/obo/GAZ_00030873">
        <obo:RO_0001025 rdf:resource="http://purl.obolibrary.org/obo/GAZ_02000744"/>
        <oboInOwl:hasOBONamespace>GAZ</oboInOwl:hasOBONamespace>
        <oboInOwl:id>GAZ:00030873</oboInOwl:id>
        <rdfs:label>Al-Mazar al-Janubiyya Subdistrict</rdfs:label>
    </owl:NamedIndividual>
    


    <!-- http://purl.obolibrary.org/obo/GAZ_00030874 -->

    <owl:NamedIndividual rdf:about="http://purl.obolibrary.org/obo/GAZ_00030874">
        <obo:RO_0001025 rdf:resource="http://purl.obolibrary.org/obo/GAZ_02000744"/>
        <oboInOwl:hasOBONamespace>GAZ</oboInOwl:hasOBONamespace>
        <oboInOwl:id>GAZ:00030874</oboInOwl:id>
        <rdfs:label>Al-Qasr Subdistrict</rdfs:label>
    </owl:NamedIndividual>
    


    <!-- http://purl.obolibrary.org/obo/GAZ_00030875 -->

    <owl:NamedIndividual rdf:about="http://purl.obolibrary.org/obo/GAZ_00030875">
        <obo:RO_0001025 rdf:resource="http://purl.obolibrary.org/obo/GAZ_02000744"/>
        <oboInOwl:hasOBONamespace>GAZ</oboInOwl:hasOBONamespace>
        <oboInOwl:id>GAZ:00030875</oboInOwl:id>
        <rdfs:label>Al-Safi Subdistrict</rdfs:label>
    </owl:NamedIndividual>
    


    <!-- http://purl.obolibrary.org/obo/GAZ_00030876 -->

    <owl:NamedIndividual rdf:about="http://purl.obolibrary.org/obo/GAZ_00030876">
        <obo:RO_0001025 rdf:resource="http://purl.obolibrary.org/obo/GAZ_02000744"/>
        <oboInOwl:hasOBONamespace>GAZ</oboInOwl:hasOBONamespace>
        <oboInOwl:id>GAZ:00030876</oboInOwl:id>
        <rdfs:label>Al-Mazra&apos;a Subdistrict</rdfs:label>
    </owl:NamedIndividual>
    


    <!-- http://purl.obolibrary.org/obo/GAZ_00030877 -->

    <owl:NamedIndividual rdf:about="http://purl.obolibrary.org/obo/GAZ_00030877">
        <obo:RO_0001025 rdf:resource="http://purl.obolibrary.org/obo/GAZ_02000744"/>
        <oboInOwl:hasOBONamespace>GAZ</oboInOwl:hasOBONamespace>
        <oboInOwl:id>GAZ:00030877</oboInOwl:id>
        <rdfs:label>Al-Karak Subdistrict</rdfs:label>
    </owl:NamedIndividual>
    


    <!-- http://purl.obolibrary.org/obo/GAZ_00030878 -->

    <owl:NamedIndividual rdf:about="http://purl.obolibrary.org/obo/GAZ_00030878">
        <obo:RO_0001025 rdf:resource="http://purl.obolibrary.org/obo/GAZ_02000744"/>
        <oboInOwl:hasOBONamespace>GAZ</oboInOwl:hasOBONamespace>
        <oboInOwl:id>GAZ:00030878</oboInOwl:id>
        <rdfs:label>Faqqu Subdistrict</rdfs:label>
    </owl:NamedIndividual>
    


    <!-- http://purl.obolibrary.org/obo/GAZ_00030879 -->

    <owl:NamedIndividual rdf:about="http://purl.obolibrary.org/obo/GAZ_00030879">
        <obo:RO_0001025 rdf:resource="http://purl.obolibrary.org/obo/GAZ_02000744"/>
        <oboInOwl:hasOBONamespace>GAZ</oboInOwl:hasOBONamespace>
        <oboInOwl:id>GAZ:00030879</oboInOwl:id>
        <rdfs:label>Ayy Subdistrict</rdfs:label>
    </owl:NamedIndividual>
    


    <!-- http://purl.obolibrary.org/obo/GAZ_00030880 -->

    <owl:NamedIndividual rdf:about="http://purl.obolibrary.org/obo/GAZ_00030880">
        <obo:RO_0001025 rdf:resource="http://purl.obolibrary.org/obo/GAZ_02000739"/>
        <oboInOwl:hasOBONamespace>GAZ</oboInOwl:hasOBONamespace>
        <oboInOwl:id>GAZ:00030880</oboInOwl:id>
        <rdfs:label>Al-Husanyniyya Subdistrict</rdfs:label>
    </owl:NamedIndividual>
    


    <!-- http://purl.obolibrary.org/obo/GAZ_00030881 -->

    <owl:NamedIndividual rdf:about="http://purl.obolibrary.org/obo/GAZ_00030881">
        <obo:RO_0001025 rdf:resource="http://purl.obolibrary.org/obo/GAZ_02000739"/>
        <oboInOwl:hasOBONamespace>GAZ</oboInOwl:hasOBONamespace>
        <oboInOwl:id>GAZ:00030881</oboInOwl:id>
        <rdfs:label>Ayi Subdistrict</rdfs:label>
    </owl:NamedIndividual>
    


    <!-- http://purl.obolibrary.org/obo/GAZ_00030882 -->

    <owl:NamedIndividual rdf:about="http://purl.obolibrary.org/obo/GAZ_00030882">
        <obo:RO_0001025 rdf:resource="http://purl.obolibrary.org/obo/GAZ_02000739"/>
        <oboInOwl:hasOBONamespace>GAZ</oboInOwl:hasOBONamespace>
        <oboInOwl:id>GAZ:00030882</oboInOwl:id>
        <rdfs:label>Wadi Mus Subdistrict</rdfs:label>
    </owl:NamedIndividual>
    


    <!-- http://purl.obolibrary.org/obo/GAZ_00030883 -->

    <owl:NamedIndividual rdf:about="http://purl.obolibrary.org/obo/GAZ_00030883">
        <obo:RO_0001025 rdf:resource="http://purl.obolibrary.org/obo/GAZ_02000739"/>
        <oboInOwl:hasOBONamespace>GAZ</oboInOwl:hasOBONamespace>
        <oboInOwl:id>GAZ:00030883</oboInOwl:id>
        <rdfs:label>Ma&apos;an Subdistrict</rdfs:label>
    </owl:NamedIndividual>
    


    <!-- http://purl.obolibrary.org/obo/GAZ_00030884 -->

    <owl:NamedIndividual rdf:about="http://purl.obolibrary.org/obo/GAZ_00030884">
        <obo:RO_0001025 rdf:resource="http://purl.obolibrary.org/obo/GAZ_02000739"/>
        <oboInOwl:hasOBONamespace>GAZ</oboInOwl:hasOBONamespace>
        <oboInOwl:id>GAZ:00030884</oboInOwl:id>
        <rdfs:label>Ash-Shibek Subdistrict</rdfs:label>
    </owl:NamedIndividual>
    


    <!-- http://purl.obolibrary.org/obo/GAZ_00030885 -->

    <owl:NamedIndividual rdf:about="http://purl.obolibrary.org/obo/GAZ_00030885">
        <obo:RO_0001025 rdf:resource="http://purl.obolibrary.org/obo/GAZ_02000741"/>
        <oboInOwl:hasOBONamespace>GAZ</oboInOwl:hasOBONamespace>
        <oboInOwl:id>GAZ:00030885</oboInOwl:id>
        <rdfs:label>Dhiban Subdistrict</rdfs:label>
    </owl:NamedIndividual>
    


    <!-- http://purl.obolibrary.org/obo/GAZ_00030886 -->

    <owl:NamedIndividual rdf:about="http://purl.obolibrary.org/obo/GAZ_00030886">
        <obo:RO_0001025 rdf:resource="http://purl.obolibrary.org/obo/GAZ_02000741"/>
        <oboInOwl:hasOBONamespace>GAZ</oboInOwl:hasOBONamespace>
        <oboInOwl:id>GAZ:00030886</oboInOwl:id>
        <rdfs:label>Madaba Subdistrict</rdfs:label>
    </owl:NamedIndividual>
    


    <!-- http://purl.obolibrary.org/obo/GAZ_00030887 -->

    <owl:NamedIndividual rdf:about="http://purl.obolibrary.org/obo/GAZ_00030887">
        <obo:RO_0001025 rdf:resource="http://purl.obolibrary.org/obo/GAZ_02000740"/>
        <oboInOwl:hasOBONamespace>GAZ</oboInOwl:hasOBONamespace>
        <oboInOwl:id>GAZ:00030887</oboInOwl:id>
        <rdfs:label>Ar-Ruwayshid Subdistrict</rdfs:label>
    </owl:NamedIndividual>
    


    <!-- http://purl.obolibrary.org/obo/GAZ_00030888 -->

    <owl:NamedIndividual rdf:about="http://purl.obolibrary.org/obo/GAZ_00030888">
        <obo:RO_0001025 rdf:resource="http://purl.obolibrary.org/obo/GAZ_02000740"/>
        <oboInOwl:hasOBONamespace>GAZ</oboInOwl:hasOBONamespace>
        <oboInOwl:id>GAZ:00030888</oboInOwl:id>
        <rdfs:label>Sabha Subdistrict</rdfs:label>
    </owl:NamedIndividual>
    


    <!-- http://purl.obolibrary.org/obo/GAZ_00030889 -->

    <owl:NamedIndividual rdf:about="http://purl.obolibrary.org/obo/GAZ_00030889">
        <obo:RO_0001025 rdf:resource="http://purl.obolibrary.org/obo/GAZ_02000740"/>
        <oboInOwl:hasOBONamespace>GAZ</oboInOwl:hasOBONamespace>
        <oboInOwl:id>GAZ:00030889</oboInOwl:id>
        <rdfs:label>Bal&apos;ama Subdistrict</rdfs:label>
    </owl:NamedIndividual>
    


    <!-- http://purl.obolibrary.org/obo/GAZ_00030890 -->

    <owl:NamedIndividual rdf:about="http://purl.obolibrary.org/obo/GAZ_00030890">
        <obo:RO_0001025 rdf:resource="http://purl.obolibrary.org/obo/GAZ_02000740"/>
        <oboInOwl:hasOBONamespace>GAZ</oboInOwl:hasOBONamespace>
        <oboInOwl:id>GAZ:00030890</oboInOwl:id>
        <rdfs:label>Al-Mafraq Subdistrict</rdfs:label>
    </owl:NamedIndividual>
    


    <!-- http://purl.obolibrary.org/obo/GAZ_00030891 -->

    <owl:NamedIndividual rdf:about="http://purl.obolibrary.org/obo/GAZ_00030891">
        <obo:RO_0001025 rdf:resource="http://purl.obolibrary.org/obo/GAZ_02000740"/>
        <oboInOwl:hasOBONamespace>GAZ</oboInOwl:hasOBONamespace>
        <oboInOwl:id>GAZ:00030891</oboInOwl:id>
        <rdfs:label>Sama as-Sarhan Subdistrict</rdfs:label>
    </owl:NamedIndividual>
    


    <!-- http://purl.obolibrary.org/obo/GAZ_00030892 -->

    <owl:NamedIndividual rdf:about="http://purl.obolibrary.org/obo/GAZ_00030892">
        <obo:RO_0001025 rdf:resource="http://purl.obolibrary.org/obo/GAZ_02000749"/>
        <oboInOwl:hasOBONamespace>GAZ</oboInOwl:hasOBONamespace>
        <oboInOwl:id>GAZ:00030892</oboInOwl:id>
        <rdfs:label>Al-Tafila Subdistrict</rdfs:label>
    </owl:NamedIndividual>
    


    <!-- http://purl.obolibrary.org/obo/GAZ_00030893 -->

    <owl:NamedIndividual rdf:about="http://purl.obolibrary.org/obo/GAZ_00030893">
        <obo:RO_0001025 rdf:resource="http://purl.obolibrary.org/obo/GAZ_02000749"/>
        <oboInOwl:hasOBONamespace>GAZ</oboInOwl:hasOBONamespace>
        <oboInOwl:id>GAZ:00030893</oboInOwl:id>
        <rdfs:label>Al-Hasa Subdistrict</rdfs:label>
    </owl:NamedIndividual>
    


    <!-- http://purl.obolibrary.org/obo/GAZ_00030894 -->

    <owl:NamedIndividual rdf:about="http://purl.obolibrary.org/obo/GAZ_00030894">
        <obo:RO_0001025 rdf:resource="http://purl.obolibrary.org/obo/GAZ_02000749"/>
        <oboInOwl:hasOBONamespace>GAZ</oboInOwl:hasOBONamespace>
        <oboInOwl:id>GAZ:00030894</oboInOwl:id>
        <rdfs:label>Birsayra Subdistrict</rdfs:label>
    </owl:NamedIndividual>
    


    <!-- http://purl.obolibrary.org/obo/GAZ_00030895 -->

    <owl:NamedIndividual rdf:about="http://purl.obolibrary.org/obo/GAZ_00030895">
        <obo:RO_0001025 rdf:resource="http://purl.obolibrary.org/obo/GAZ_02000748"/>
        <oboInOwl:hasOBONamespace>GAZ</oboInOwl:hasOBONamespace>
        <oboInOwl:id>GAZ:00030895</oboInOwl:id>
        <rdfs:label>Al-Azraq Subdistrict</rdfs:label>
    </owl:NamedIndividual>
    


    <!-- http://purl.obolibrary.org/obo/GAZ_00030896 -->

    <owl:NamedIndividual rdf:about="http://purl.obolibrary.org/obo/GAZ_00030896">
        <obo:RO_0001025 rdf:resource="http://purl.obolibrary.org/obo/GAZ_02000748"/>
        <oboInOwl:hasOBONamespace>GAZ</oboInOwl:hasOBONamespace>
        <oboInOwl:id>GAZ:00030896</oboInOwl:id>
        <rdfs:label>Az-Zarqa Subdistrict</rdfs:label>
    </owl:NamedIndividual>
    


    <!-- http://purl.obolibrary.org/obo/GAZ_00030897 -->

    <owl:NamedIndividual rdf:about="http://purl.obolibrary.org/obo/GAZ_00030897">
        <obo:RO_0001025 rdf:resource="http://purl.obolibrary.org/obo/GAZ_02000748"/>
        <oboInOwl:hasOBONamespace>GAZ</oboInOwl:hasOBONamespace>
        <oboInOwl:id>GAZ:00030897</oboInOwl:id>
        <rdfs:label>Birin Subdistrict</rdfs:label>
    </owl:NamedIndividual>
    


    <!-- http://purl.obolibrary.org/obo/GAZ_00044914 -->

    <owl:NamedIndividual rdf:about="http://purl.obolibrary.org/obo/GAZ_00044914">
        <obo:RO_0001025 rdf:resource="http://purl.obolibrary.org/obo/GAZ_00007520"/>
        <obo:IAO_0000115>A freshwater monomictic lake, being approximately 53 km in circumference, about 21 km long, and 13 km wide. The lake has a total area of 166 km2, and a maximum depth of approximately 43 m. It is situated deep in the Jordan Great Rift Valley, the valley caused by the separation of the African and Arabian Plates and is fed partly by underground springs although its main source is the Jordan River which flows through it from north to south. Consequently the area is subject to earthquakes and, in the past, volcanic activity. This is evidenced by the abundant basalt and other igneous rocks that define the geology of the Galilee region.</obo:IAO_0000115>
        <oboInOwl:hasOBONamespace>GAZ</oboInOwl:hasOBONamespace>
        <oboInOwl:id>GAZ:00044914</oboInOwl:id>
        <rdfs:label>Sea of Galilee</rdfs:label>
    </owl:NamedIndividual>
    


    <!-- http://purl.obolibrary.org/obo/GAZ_00044915 -->

    <owl:NamedIndividual rdf:about="http://purl.obolibrary.org/obo/GAZ_00044915">
        <obo:IAO_0000115>A 375 km long strike-slip fault zone some 5 km wide in the north and 23 km wide in the south that forms part of the broader Great Rift Valley. Located in modern-day Israel, Jordan, the West Bank and the Golan Heights, this geographic region includes the Jordan River, Hula Valley, Lake Tiberias and the Dead Sea, features created by the physiographic and geologic process underway.</obo:IAO_0000115>
        <oboInOwl:hasOBONamespace>GAZ</oboInOwl:hasOBONamespace>
        <oboInOwl:id>GAZ:00044915</oboInOwl:id>
        <rdfs:label>Jordan Rift Valley</rdfs:label>
    </owl:NamedIndividual>
    


    <!-- http://purl.obolibrary.org/obo/GAZ_00044916 -->

    <owl:NamedIndividual rdf:about="http://purl.obolibrary.org/obo/GAZ_00044916">
        <obo:RO_0001025 rdf:resource="http://purl.obolibrary.org/obo/GAZ_00044915"/>
        <obo:IAO_0000115>A section of the Great Rift Valley lying between the Dead Sea to the north and the Gulf of Aqaba or the Gulf of Eilat to the south. It forms part of the border between Israel to the west and Jordan to the east.</obo:IAO_0000115>
        <oboInOwl:hasOBONamespace>GAZ</oboInOwl:hasOBONamespace>
        <oboInOwl:id>GAZ:00044916</oboInOwl:id>
        <rdfs:label>Wadi Arabah</rdfs:label>
    </owl:NamedIndividual>
    


    <!-- http://purl.obolibrary.org/obo/GAZ_00049007 -->

    <owl:NamedIndividual rdf:about="http://purl.obolibrary.org/obo/GAZ_00049007">
        <obo:RO_0001025 rdf:resource="http://purl.obolibrary.org/obo/GAZ_00007862"/>
        <obo:IAO_0000115>The narrow sea passages, about 13 km wide, between the Sinai and Arabian peninsulas which separates the Gulf of Aqaba from the Red Sea.</obo:IAO_0000115>
        <oboInOwl:hasOBONamespace>GAZ</oboInOwl:hasOBONamespace>
        <oboInOwl:id>GAZ:00049007</oboInOwl:id>
        <rdfs:label>Straits of Tiran</rdfs:label>
    </owl:NamedIndividual>
    


    <!-- http://purl.obolibrary.org/obo/GAZ_00049008 -->

    <owl:NamedIndividual rdf:about="http://purl.obolibrary.org/obo/GAZ_00049008">
        <obo:RO_0001025 rdf:resource="http://purl.obolibrary.org/obo/GAZ_00049007"/>
        <obo:IAO_0000115>A Saudi Arabian island in the Straits of Tiran east of Tiran Island.</obo:IAO_0000115>
        <oboInOwl:hasOBONamespace>GAZ</oboInOwl:hasOBONamespace>
        <oboInOwl:id>GAZ:00049008</oboInOwl:id>
        <rdfs:label>Sanafir Island</rdfs:label>
    </owl:NamedIndividual>
    


    <!-- http://purl.obolibrary.org/obo/GAZ_00049009 -->

    <owl:NamedIndividual rdf:about="http://purl.obolibrary.org/obo/GAZ_00049009">
        <obo:RO_0001025 rdf:resource="http://purl.obolibrary.org/obo/GAZ_00049007"/>
        <obo:IAO_0000115>An island belonging to Saudi Arabia at the entrance of the Straits of Tiran, which separates the Red Sea and the Gulf of Aqaba.</obo:IAO_0000115>
        <oboInOwl:hasOBONamespace>GAZ</oboInOwl:hasOBONamespace>
        <oboInOwl:id>GAZ:00049009</oboInOwl:id>
        <rdfs:label>Tiran Island</rdfs:label>
    </owl:NamedIndividual>
    


    <!-- http://purl.obolibrary.org/obo/GAZ_00052877 -->

    <owl:NamedIndividual rdf:about="http://purl.obolibrary.org/obo/GAZ_00052877">
        <obo:RO_0001025 rdf:resource="http://purl.obolibrary.org/obo/GAZ_00030877"/>
        <obo:IAO_0000115>A populated place.</obo:IAO_0000115>
        <oboInOwl:hasOBONamespace>GAZ</oboInOwl:hasOBONamespace>
        <oboInOwl:id>GAZ:00052877</oboInOwl:id>
        <rdfs:label>Al Qatrana</rdfs:label>
    </owl:NamedIndividual>
    


    <!-- http://purl.obolibrary.org/obo/GAZ_00052878 -->

    <owl:NamedIndividual rdf:about="http://purl.obolibrary.org/obo/GAZ_00052878">
        <obo:RO_0001025 rdf:resource="http://purl.obolibrary.org/obo/GAZ_00030853"/>
        <obo:IAO_0000115>A city that is the capital of the Hashemite Kingdom of Jordan.</obo:IAO_0000115>
        <oboInOwl:hasOBONamespace>GAZ</oboInOwl:hasOBONamespace>
        <oboInOwl:id>GAZ:00052878</oboInOwl:id>
        <rdfs:label>Amman</rdfs:label>
    </owl:NamedIndividual>
    


    <!-- http://purl.obolibrary.org/obo/GAZ_00052879 -->

    <owl:NamedIndividual rdf:about="http://purl.obolibrary.org/obo/GAZ_00052879">
        <obo:RO_0001025 rdf:resource="http://purl.obolibrary.org/obo/GAZ_00030856"/>
        <obo:IAO_0000115>A coastal town in the far south of Jordan. It is the capital of Aqaba Governorate.</obo:IAO_0000115>
        <oboInOwl:hasOBONamespace>GAZ</oboInOwl:hasOBONamespace>
        <oboInOwl:id>GAZ:00052879</oboInOwl:id>
        <rdfs:label>Aqaba</rdfs:label>
    </owl:NamedIndividual>
    


    <!-- http://purl.obolibrary.org/obo/GAZ_00052881 -->

    <owl:NamedIndividual rdf:about="http://purl.obolibrary.org/obo/GAZ_00052881">
        <obo:RO_0001025 rdf:resource="http://purl.obolibrary.org/obo/GAZ_00030857"/>
        <obo:IAO_0000115>An archaeological site in southwestern Jordan, lying on the slope of Mount Hor in a basin among the mountains which form the eastern flank of Arabah (Wadi Araba), the large valley running from the Dead Sea to the Gulf of Aqaba.</obo:IAO_0000115>
        <oboInOwl:hasOBONamespace>GAZ</oboInOwl:hasOBONamespace>
        <oboInOwl:id>GAZ:00052881</oboInOwl:id>
        <rdfs:label>Petra</rdfs:label>
    </owl:NamedIndividual>
    


    <!-- http://purl.obolibrary.org/obo/GAZ_00052883 -->

    <owl:NamedIndividual rdf:about="http://purl.obolibrary.org/obo/GAZ_00052883">
        <obo:IAO_0000115>A dam on the Yarmuk River.</obo:IAO_0000115>
        <oboInOwl:hasOBONamespace>GAZ</oboInOwl:hasOBONamespace>
        <oboInOwl:id>GAZ:00052883</oboInOwl:id>
        <rdfs:label>Maqarin Dam</rdfs:label>
    </owl:NamedIndividual>
    


    <!-- http://purl.obolibrary.org/obo/GAZ_00052884 -->

    <owl:NamedIndividual rdf:about="http://purl.obolibrary.org/obo/GAZ_00052884">
        <obo:RO_0001025 rdf:resource="http://purl.obolibrary.org/obo/GAZ_02000743"/>
        <obo:IAO_0000115>A region in N Jordon near the Yarmuk River where bitumen has burned and pyrometamorphosed limestone to natural cement.</obo:IAO_0000115>
        <oboInOwl:hasOBONamespace>GAZ</oboInOwl:hasOBONamespace>
        <oboInOwl:id>GAZ:00052884</oboInOwl:id>
        <rdfs:label>Maqarin</rdfs:label>
    </owl:NamedIndividual>
    


    <!-- http://purl.obolibrary.org/obo/GAZ_00052885 -->

    <owl:NamedIndividual rdf:about="http://purl.obolibrary.org/obo/GAZ_00052885">
        <obo:RO_0001025 rdf:resource="http://purl.obolibrary.org/obo/GAZ_00030872"/>
        <obo:IAO_0000115>A city thatis the capital of Jerash Governorate.</obo:IAO_0000115>
        <oboInOwl:hasOBONamespace>GAZ</oboInOwl:hasOBONamespace>
        <oboInOwl:id>GAZ:00052885</oboInOwl:id>
        <rdfs:label>Jerash</rdfs:label>
    </owl:NamedIndividual>
    


    <!-- http://purl.obolibrary.org/obo/GAZ_00052886 -->

    <owl:NamedIndividual rdf:about="http://purl.obolibrary.org/obo/GAZ_00052886">
        <rdf:type rdf:resource="http://purl.obolibrary.org/obo/ENVO_00000856"/>
        <obo:RO_0001025 rdf:resource="http://purl.obolibrary.org/obo/GAZ_02000749"/>
        <obo:IAO_0000115>A small village near the city of Tafilah, in central-western Jordan. It is situated on the edge of a large natural gorge, Wadi Dana.</obo:IAO_0000115>
        <oboInOwl:hasOBONamespace>GAZ</oboInOwl:hasOBONamespace>
        <oboInOwl:id>GAZ:00052886</oboInOwl:id>
        <rdfs:label>Dana</rdfs:label>
    </owl:NamedIndividual>
    


    <!-- http://purl.obolibrary.org/obo/GAZ_00052887 -->

    <owl:NamedIndividual rdf:about="http://purl.obolibrary.org/obo/GAZ_00052887">
        <obo:RO_0001025 rdf:resource="http://purl.obolibrary.org/obo/GAZ_00030866"/>
        <obo:IAO_0000115>A populated place. A city in Jordan located about 70 km north of Amman on the northern ridge of the Gilead.</obo:IAO_0000115>
        <oboInOwl:hasOBONamespace>GAZ</oboInOwl:hasOBONamespace>
        <oboInOwl:id>GAZ:00052887</oboInOwl:id>
        <rdfs:label>Irbid</rdfs:label>
    </owl:NamedIndividual>
    


    <!-- http://purl.obolibrary.org/obo/GAZ_00052888 -->

    <owl:NamedIndividual rdf:about="http://purl.obolibrary.org/obo/GAZ_00052888">
        <obo:RO_0001025 rdf:resource="http://purl.obolibrary.org/obo/GAZ_02000743"/>
        <obo:IAO_0000115>A mountainous region east of the Jordan river.</obo:IAO_0000115>
        <oboInOwl:hasOBONamespace>GAZ</oboInOwl:hasOBONamespace>
        <oboInOwl:id>GAZ:00052888</oboInOwl:id>
        <rdfs:label>Gilead</rdfs:label>
    </owl:NamedIndividual>
    


    <!-- http://purl.obolibrary.org/obo/GAZ_00052889 -->

    <owl:NamedIndividual rdf:about="http://purl.obolibrary.org/obo/GAZ_00052889">
        <obo:RO_0001025 rdf:resource="http://purl.obolibrary.org/obo/GAZ_02000743"/>
        <obo:IAO_0000115>A populated place.</obo:IAO_0000115>
        <oboInOwl:hasOBONamespace>GAZ</oboInOwl:hasOBONamespace>
        <oboInOwl:id>GAZ:00052889</oboInOwl:id>
        <rdfs:label>Zubiya</rdfs:label>
    </owl:NamedIndividual>
    


    <!-- http://purl.obolibrary.org/obo/GAZ_00053683 -->

    <owl:NamedIndividual rdf:about="http://purl.obolibrary.org/obo/GAZ_00053683">
        <obo:IAO_0000115>A volcanic field in the Anti-Lebanon Mountains of SW Syria near the borders with Lebanon and Israel contains numerous cinder cones of Pliocene-to-Holocene age. The Golan Heights volcanic field covers a broad area NE of the Lake Tiberius (the Sea of Galilee) and SW of the city of Damascus (Dimashq) and includes the prehistoric cone of Majdel Shams in the Golan Heights. The volcanic field lies on a basaltic plateau that dips to the west and SW, with steep slopes facing the Dead Sea rift valley. It lies within the northern part of the massive alkaline Harrat Ash Shaam volcanic field that extends from southern Syria through NW Jordan to Saudi Arabia.</obo:IAO_0000115>
        <oboInOwl:hasOBONamespace>GAZ</oboInOwl:hasOBONamespace>
        <oboInOwl:id>GAZ:00053683</oboInOwl:id>
        <rdfs:label>Golan Heights Volcanic Field</rdfs:label>
    </owl:NamedIndividual>
    


    <!-- http://purl.obolibrary.org/obo/GAZ_00053684 -->

    <owl:NamedIndividual rdf:about="http://purl.obolibrary.org/obo/GAZ_00053684">
        <obo:IAO_0000115>A volcanic field, in southern Syria SE of the capital city of Damascas (Dimashq), consists of a lava field with broad areas containing Holocene volcanic vents. The basaltic field contains numerous vents erupted from NW-SE-trending fissures. A boiling lava lake was observed in the Es Safa volcanic area in the middle of the 19th century. This volcanic field lies within the northern part of the massive alkaline Harrat Ash Shaam volcanic field that extends from southern Syria through NE Jordan to Saudi Arabia.</obo:IAO_0000115>
        <oboInOwl:hasOBONamespace>GAZ</oboInOwl:hasOBONamespace>
        <oboInOwl:id>GAZ:00053684</oboInOwl:id>
        <rdfs:label>Es Safa Volcanic Field</rdfs:label>
    </owl:NamedIndividual>
    


    <!-- http://purl.obolibrary.org/obo/GAZ_00053685 -->

    <owl:NamedIndividual rdf:about="http://purl.obolibrary.org/obo/GAZ_00053685">
        <obo:IAO_0000115>A lava region in southern Syria. It lies about 65 km east of Damascus, located in the central part of the administrative district of Muhafazat Rif Dimashq.</obo:IAO_0000115>
        <oboInOwl:hasOBONamespace>GAZ</oboInOwl:hasOBONamespace>
        <oboInOwl:id>GAZ:00053685</oboInOwl:id>
        <rdfs:label>Dirat at Tulul</rdfs:label>
    </owl:NamedIndividual>
    


    <!-- http://purl.obolibrary.org/obo/GAZ_00053686 -->

    <owl:NamedIndividual rdf:about="http://purl.obolibrary.org/obo/GAZ_00053686">
        <obo:RO_0001025 rdf:resource="http://purl.obolibrary.org/obo/GAZ_00014012"/>
        <obo:IAO_0000115>The most prominent feature of Jabal ad Druze Volcanic Field.</obo:IAO_0000115>
        <oboInOwl:hasOBONamespace>GAZ</oboInOwl:hasOBONamespace>
        <oboInOwl:id>GAZ:00053686</oboInOwl:id>
        <rdfs:label>Jabal ad Druze Volcano</rdfs:label>
    </owl:NamedIndividual>
    


    <!-- http://purl.obolibrary.org/obo/GAZ_00053688 -->

    <owl:NamedIndividual rdf:about="http://purl.obolibrary.org/obo/GAZ_00053688">
        <obo:RO_0001025 rdf:resource="http://purl.obolibrary.org/obo/GAZ_00053685"/>
        <obo:IAO_0000115>A volcanic cone.</obo:IAO_0000115>
        <oboInOwl:hasOBONamespace>GAZ</oboInOwl:hasOBONamespace>
        <oboInOwl:id>GAZ:00053688</oboInOwl:id>
        <rdfs:label>Tell Um el Meza</rdfs:label>
    </owl:NamedIndividual>
    


    <!-- http://purl.obolibrary.org/obo/GAZ_00053689 -->

    <owl:NamedIndividual rdf:about="http://purl.obolibrary.org/obo/GAZ_00053689">
        <obo:RO_0001025 rdf:resource="http://purl.obolibrary.org/obo/GAZ_00053685"/>
        <obo:IAO_0000115>A volcanic cone.</obo:IAO_0000115>
        <oboInOwl:hasOBONamespace>GAZ</oboInOwl:hasOBONamespace>
        <oboInOwl:id>GAZ:00053689</oboInOwl:id>
        <rdfs:label>Tell Salman</rdfs:label>
    </owl:NamedIndividual>
    


    <!-- http://purl.obolibrary.org/obo/GAZ_00053690 -->

    <owl:NamedIndividual rdf:about="http://purl.obolibrary.org/obo/GAZ_00053690">
        <obo:RO_0001025 rdf:resource="http://purl.obolibrary.org/obo/GAZ_00053685"/>
        <obo:IAO_0000115>A volcanic cone.</obo:IAO_0000115>
        <oboInOwl:hasOBONamespace>GAZ</oboInOwl:hasOBONamespace>
        <oboInOwl:id>GAZ:00053690</oboInOwl:id>
        <rdfs:label>Tell Aajer</rdfs:label>
    </owl:NamedIndividual>
    


    <!-- http://purl.obolibrary.org/obo/GAZ_00053691 -->

    <owl:NamedIndividual rdf:about="http://purl.obolibrary.org/obo/GAZ_00053691">
        <obo:RO_0001025 rdf:resource="http://purl.obolibrary.org/obo/GAZ_00053685"/>
        <obo:IAO_0000115>A volcanic cone.</obo:IAO_0000115>
        <oboInOwl:hasOBONamespace>GAZ</oboInOwl:hasOBONamespace>
        <oboInOwl:id>GAZ:00053691</oboInOwl:id>
        <rdfs:label>Tell Maqhool</rdfs:label>
    </owl:NamedIndividual>
    


    <!-- http://purl.obolibrary.org/obo/GAZ_00053692 -->

    <owl:NamedIndividual rdf:about="http://purl.obolibrary.org/obo/GAZ_00053692">
        <obo:RO_0001025 rdf:resource="http://purl.obolibrary.org/obo/GAZ_00053685"/>
        <obo:IAO_0000115>A volcanic cone.</obo:IAO_0000115>
        <oboInOwl:hasOBONamespace>GAZ</oboInOwl:hasOBONamespace>
        <oboInOwl:id>GAZ:00053692</oboInOwl:id>
        <rdfs:label>Tell Daqwa</rdfs:label>
    </owl:NamedIndividual>
    


    <!-- http://purl.obolibrary.org/obo/GAZ_00053693 -->

    <owl:NamedIndividual rdf:about="http://purl.obolibrary.org/obo/GAZ_00053693">
        <obo:RO_0001025 rdf:resource="http://purl.obolibrary.org/obo/GAZ_00053685"/>
        <obo:IAO_0000115>A volcanic cone.</obo:IAO_0000115>
        <oboInOwl:hasOBONamespace>GAZ</oboInOwl:hasOBONamespace>
        <oboInOwl:id>GAZ:00053693</oboInOwl:id>
        <rdfs:label>Tell Um Masarja</rdfs:label>
    </owl:NamedIndividual>
    


    <!-- http://purl.obolibrary.org/obo/GAZ_00053694 -->

    <owl:NamedIndividual rdf:about="http://purl.obolibrary.org/obo/GAZ_00053694">
        <obo:RO_0001025 rdf:resource="http://purl.obolibrary.org/obo/GAZ_00053685"/>
        <obo:IAO_0000115>A volcanic cone.</obo:IAO_0000115>
        <oboInOwl:hasOBONamespace>GAZ</oboInOwl:hasOBONamespace>
        <oboInOwl:id>GAZ:00053694</oboInOwl:id>
        <rdfs:label>Tell El Matalla</rdfs:label>
    </owl:NamedIndividual>
    


    <!-- http://purl.obolibrary.org/obo/GAZ_00053695 -->

    <owl:NamedIndividual rdf:about="http://purl.obolibrary.org/obo/GAZ_00053695">
        <obo:RO_0001025 rdf:resource="http://purl.obolibrary.org/obo/GAZ_00053685"/>
        <obo:IAO_0000115>A volcanic cone.</obo:IAO_0000115>
        <oboInOwl:hasOBONamespace>GAZ</oboInOwl:hasOBONamespace>
        <oboInOwl:id>GAZ:00053695</oboInOwl:id>
        <rdfs:label>Tell Wastani</rdfs:label>
    </owl:NamedIndividual>
    


    <!-- http://purl.obolibrary.org/obo/GAZ_00053696 -->

    <owl:NamedIndividual rdf:about="http://purl.obolibrary.org/obo/GAZ_00053696">
        <obo:RO_0001025 rdf:resource="http://purl.obolibrary.org/obo/GAZ_00053685"/>
        <obo:IAO_0000115>A volcanic cone.</obo:IAO_0000115>
        <oboInOwl:hasOBONamespace>GAZ</oboInOwl:hasOBONamespace>
        <oboInOwl:id>GAZ:00053696</oboInOwl:id>
        <rdfs:label>Tell Um Otek</rdfs:label>
    </owl:NamedIndividual>
    


    <!-- http://purl.obolibrary.org/obo/GAZ_00053697 -->

    <owl:NamedIndividual rdf:about="http://purl.obolibrary.org/obo/GAZ_00053697">
        <obo:RO_0001025 rdf:resource="http://purl.obolibrary.org/obo/GAZ_00053685"/>
        <obo:IAO_0000115>A volcanic cone.</obo:IAO_0000115>
        <oboInOwl:hasOBONamespace>GAZ</oboInOwl:hasOBONamespace>
        <oboInOwl:id>GAZ:00053697</oboInOwl:id>
        <rdfs:label>Tell Abu Safa</rdfs:label>
    </owl:NamedIndividual>
    


    <!-- http://purl.obolibrary.org/obo/GAZ_00053698 -->

    <owl:NamedIndividual rdf:about="http://purl.obolibrary.org/obo/GAZ_00053698">
        <obo:RO_0001025 rdf:resource="http://purl.obolibrary.org/obo/GAZ_00053685"/>
        <obo:IAO_0000115>A volcanic cone.</obo:IAO_0000115>
        <oboInOwl:hasOBONamespace>GAZ</oboInOwl:hasOBONamespace>
        <oboInOwl:id>GAZ:00053698</oboInOwl:id>
        <rdfs:label>Tell Jaafar</rdfs:label>
    </owl:NamedIndividual>
    


    <!-- http://purl.obolibrary.org/obo/GAZ_00053699 -->

    <owl:NamedIndividual rdf:about="http://purl.obolibrary.org/obo/GAZ_00053699">
        <obo:RO_0001025 rdf:resource="http://purl.obolibrary.org/obo/GAZ_00053685"/>
        <obo:IAO_0000115>A volcanic cone.</obo:IAO_0000115>
        <oboInOwl:hasOBONamespace>GAZ</oboInOwl:hasOBONamespace>
        <oboInOwl:id>GAZ:00053699</oboInOwl:id>
        <rdfs:label>Tell Shayaba</rdfs:label>
    </owl:NamedIndividual>
    


    <!-- http://purl.obolibrary.org/obo/GAZ_00053700 -->

    <owl:NamedIndividual rdf:about="http://purl.obolibrary.org/obo/GAZ_00053700">
        <obo:RO_0001025 rdf:resource="http://purl.obolibrary.org/obo/GAZ_00053685"/>
        <obo:IAO_0000115>A volcanic cone.</obo:IAO_0000115>
        <oboInOwl:hasOBONamespace>GAZ</oboInOwl:hasOBONamespace>
        <oboInOwl:id>GAZ:00053700</oboInOwl:id>
        <rdfs:label>Tell Khneifes</rdfs:label>
    </owl:NamedIndividual>
    


    <!-- http://purl.obolibrary.org/obo/GAZ_00053701 -->

    <owl:NamedIndividual rdf:about="http://purl.obolibrary.org/obo/GAZ_00053701">
        <obo:RO_0001025 rdf:resource="http://purl.obolibrary.org/obo/GAZ_00053685"/>
        <obo:IAO_0000115>A volcanic cone.</obo:IAO_0000115>
        <oboInOwl:hasOBONamespace>GAZ</oboInOwl:hasOBONamespace>
        <oboInOwl:id>GAZ:00053701</oboInOwl:id>
        <rdfs:label>Tell Hweijer</rdfs:label>
    </owl:NamedIndividual>
    


    <!-- http://purl.obolibrary.org/obo/GAZ_00053702 -->

    <owl:NamedIndividual rdf:about="http://purl.obolibrary.org/obo/GAZ_00053702">
        <obo:RO_0001025 rdf:resource="http://purl.obolibrary.org/obo/GAZ_00053685"/>
        <obo:IAO_0000115>A volcanic cone.</obo:IAO_0000115>
        <oboInOwl:hasOBONamespace>GAZ</oboInOwl:hasOBONamespace>
        <oboInOwl:id>GAZ:00053702</oboInOwl:id>
        <rdfs:label>Tell Shimali</rdfs:label>
    </owl:NamedIndividual>
    


    <!-- http://purl.obolibrary.org/obo/GAZ_00053703 -->

    <owl:NamedIndividual rdf:about="http://purl.obolibrary.org/obo/GAZ_00053703">
        <obo:RO_0001025 rdf:resource="http://purl.obolibrary.org/obo/GAZ_00053685"/>
        <obo:IAO_0000115>A volcanic cone.</obo:IAO_0000115>
        <oboInOwl:hasOBONamespace>GAZ</oboInOwl:hasOBONamespace>
        <oboInOwl:id>GAZ:00053703</oboInOwl:id>
        <rdfs:label>Tell Hweimel</rdfs:label>
    </owl:NamedIndividual>
    


    <!-- http://purl.obolibrary.org/obo/GAZ_00053704 -->

    <owl:NamedIndividual rdf:about="http://purl.obolibrary.org/obo/GAZ_00053704">
        <obo:RO_0001025 rdf:resource="http://purl.obolibrary.org/obo/GAZ_00053685"/>
        <obo:IAO_0000115>A volcanic cone.</obo:IAO_0000115>
        <oboInOwl:hasOBONamespace>GAZ</oboInOwl:hasOBONamespace>
        <oboInOwl:id>GAZ:00053704</oboInOwl:id>
        <rdfs:label>Tell el Antoor</rdfs:label>
    </owl:NamedIndividual>
    


    <!-- http://purl.obolibrary.org/obo/GAZ_00053705 -->

    <owl:NamedIndividual rdf:about="http://purl.obolibrary.org/obo/GAZ_00053705">
        <obo:RO_0001025 rdf:resource="http://purl.obolibrary.org/obo/GAZ_00053685"/>
        <obo:IAO_0000115>A volcanic cone.</obo:IAO_0000115>
        <oboInOwl:hasOBONamespace>GAZ</oboInOwl:hasOBONamespace>
        <oboInOwl:id>GAZ:00053705</oboInOwl:id>
        <rdfs:label>Tell Um Rqeibi</rdfs:label>
    </owl:NamedIndividual>
    


    <!-- http://purl.obolibrary.org/obo/GAZ_00053706 -->

    <owl:NamedIndividual rdf:about="http://purl.obolibrary.org/obo/GAZ_00053706">
        <obo:RO_0001025 rdf:resource="http://purl.obolibrary.org/obo/GAZ_00053685"/>
        <obo:IAO_0000115>A volcanic cone.</obo:IAO_0000115>
        <oboInOwl:hasOBONamespace>GAZ</oboInOwl:hasOBONamespace>
        <oboInOwl:id>GAZ:00053706</oboInOwl:id>
        <rdfs:label>Tell Qebli</rdfs:label>
    </owl:NamedIndividual>
    


    <!-- http://purl.obolibrary.org/obo/GAZ_00053707 -->

    <owl:NamedIndividual rdf:about="http://purl.obolibrary.org/obo/GAZ_00053707">
        <obo:RO_0001025 rdf:resource="http://purl.obolibrary.org/obo/GAZ_00053685"/>
        <obo:IAO_0000115>A volcanic cone.</obo:IAO_0000115>
        <oboInOwl:hasOBONamespace>GAZ</oboInOwl:hasOBONamespace>
        <oboInOwl:id>GAZ:00053707</oboInOwl:id>
        <rdfs:label>Tell As Skhana</rdfs:label>
    </owl:NamedIndividual>
    


    <!-- http://purl.obolibrary.org/obo/GAZ_00053708 -->

    <owl:NamedIndividual rdf:about="http://purl.obolibrary.org/obo/GAZ_00053708">
        <obo:IAO_0000115>A large basaltic volcanic field in northwestern Saudi Arabia near the Jordanian border, covers an area of 15,200 sq km. The volcanic field forms the southern third of the massive Harrat Ash Shamah volcanic field, which extends from Syria through Jordan into northern Saudi Arabia. The Saudi Arabian portion of the Harrat Ash Shamah volcanic field extends across a 210 km-long, roughly 75 km wide NW-SE-trending area on the NE flanks of the Wadi Sirhan and reaches its 1100 m high point at Jabal al Amud.</obo:IAO_0000115>
        <oboInOwl:hasOBONamespace>GAZ</oboInOwl:hasOBONamespace>
        <oboInOwl:id>GAZ:00053708</oboInOwl:id>
        <rdfs:label>Al Harrah Volcanic Field</rdfs:label>
    </owl:NamedIndividual>
    


    <!-- http://purl.obolibrary.org/obo/GAZ_00058383 -->

    <owl:NamedIndividual rdf:about="http://purl.obolibrary.org/obo/GAZ_00058383">
        <obo:RO_0001025 rdf:resource="http://purl.obolibrary.org/obo/GAZ_00053683"/>
        <obo:IAO_0000115>A crater lake in the northeastern Golan Heights, near Mount Hermon.</obo:IAO_0000115>
        <oboInOwl:hasOBONamespace>GAZ</oboInOwl:hasOBONamespace>
        <oboInOwl:id>GAZ:00058383</oboInOwl:id>
        <rdfs:label>Birkat Ram</rdfs:label>
    </owl:NamedIndividual>
    


    <!-- http://purl.obolibrary.org/obo/GAZ_00058384 -->

    <owl:NamedIndividual rdf:about="http://purl.obolibrary.org/obo/GAZ_00058384">
        <obo:RO_0001025 rdf:resource="http://purl.obolibrary.org/obo/GAZ_00008742"/>
        <obo:IAO_0000115>A lake that was drained in the 1950s, but is now being regenerated.</obo:IAO_0000115>
        <oboInOwl:hasOBONamespace>GAZ</oboInOwl:hasOBONamespace>
        <oboInOwl:id>GAZ:00058384</oboInOwl:id>
        <rdfs:label>Lake Hulah</rdfs:label>
    </owl:NamedIndividual>
    


    <!-- http://purl.obolibrary.org/obo/GAZ_00176005 -->

    <owl:NamedIndividual rdf:about="http://purl.obolibrary.org/obo/GAZ_00176005">
        <obo:RO_0001025 rdf:resource="http://purl.obolibrary.org/obo/GAZ_00007862"/>
        <obo:IAO_0000115>An island in the northern Gulf of Aqaba off the shore of Egypt&apos;s eastern Sinai Peninsula.</obo:IAO_0000115>
        <oboInOwl:hasOBONamespace>GAZ</oboInOwl:hasOBONamespace>
        <oboInOwl:id>GAZ:00176005</oboInOwl:id>
        <rdfs:label>Pharaoh&apos;s Island</rdfs:label>
    </owl:NamedIndividual>
    


    <!-- http://purl.obolibrary.org/obo/GAZ_00193785 -->

    <owl:NamedIndividual rdf:about="http://purl.obolibrary.org/obo/GAZ_00193785">
        <obo:RO_0001025 rdf:resource="http://purl.obolibrary.org/obo/GAZ_00007520"/>
        <obo:IAO_0000115>A river. A tributary of the Jordan River.</obo:IAO_0000115>
        <oboInOwl:hasOBONamespace>GAZ</oboInOwl:hasOBONamespace>
        <oboInOwl:id>GAZ:00193785</oboInOwl:id>
        <rdfs:label>Banias River</rdfs:label>
    </owl:NamedIndividual>
    


    <!-- http://purl.obolibrary.org/obo/GAZ_00193791 -->

    <owl:NamedIndividual rdf:about="http://purl.obolibrary.org/obo/GAZ_00193791">
        <obo:IAO_0000115>The lowest nature reserve in the world, with a spectacular array of scenery near the east cost of the Dead Sea. The reserve is located within the deep Wadi Mujib gorge, which enters the Dead Sea at 410 m below sea level. The Reserve extends to the Kerak and Madaba mountains to the north and south.</obo:IAO_0000115>
        <oboInOwl:hasOBONamespace>GAZ</oboInOwl:hasOBONamespace>
        <oboInOwl:id>GAZ:00193791</oboInOwl:id>
        <rdfs:label>Mujib Nature Reserve</rdfs:label>
    </owl:NamedIndividual>
    


    <!-- http://purl.obolibrary.org/obo/GAZ_00193792 -->

    <owl:NamedIndividual rdf:about="http://purl.obolibrary.org/obo/GAZ_00193792">
        <obo:RO_0001025 rdf:resource="http://purl.obolibrary.org/obo/GAZ_02000747"/>
        <obo:IAO_0000115>A protected area. Established 1975.</obo:IAO_0000115>
        <oboInOwl:hasOBONamespace>GAZ</oboInOwl:hasOBONamespace>
        <oboInOwl:id>GAZ:00193792</oboInOwl:id>
        <rdfs:label>Shawmari Wildlife Reserve</rdfs:label>
    </owl:NamedIndividual>
    


    <!-- http://purl.obolibrary.org/obo/GAZ_00193793 -->

    <owl:NamedIndividual rdf:about="http://purl.obolibrary.org/obo/GAZ_00193793">
        <obo:RO_0001025 rdf:resource="http://purl.obolibrary.org/obo/GAZ_00052886"/>
        <obo:IAO_0000115>A protected area. It is composed of a chain of valleys and mountains which extend from the top of the Jordan Rift Valley down to the desert lowlands of Wadi Araba. Established 1989.</obo:IAO_0000115>
        <oboInOwl:hasOBONamespace>GAZ</oboInOwl:hasOBONamespace>
        <oboInOwl:id>GAZ:00193793</oboInOwl:id>
        <rdfs:label>Dana Nature Reserve</rdfs:label>
    </owl:NamedIndividual>
    


    <!-- http://purl.obolibrary.org/obo/GAZ_00193794 -->

    <owl:NamedIndividual rdf:about="http://purl.obolibrary.org/obo/GAZ_00193794">
        <obo:RO_0001025 rdf:resource="http://purl.obolibrary.org/obo/GAZ_02000748"/>
        <obo:IAO_0000115>A protected area. Established 1978. A Ramsar Site.</obo:IAO_0000115>
        <oboInOwl:hasOBONamespace>GAZ</oboInOwl:hasOBONamespace>
        <oboInOwl:id>GAZ:00193794</oboInOwl:id>
        <rdfs:label>Azraq Wetland Reserve</rdfs:label>
    </owl:NamedIndividual>
    


    <!-- http://purl.obolibrary.org/obo/GAZ_00193795 -->

    <owl:NamedIndividual rdf:about="http://purl.obolibrary.org/obo/GAZ_00193795">
        <rdf:type rdf:resource="http://purl.obolibrary.org/obo/ENVO_00000196"/>
        <obo:RO_0001025 rdf:resource="http://purl.obolibrary.org/obo/GAZ_00251598"/>
        <obo:IAO_0000115>A seasonally flooded mudlfat. A playa.</obo:IAO_0000115>
        <oboInOwl:hasOBONamespace>GAZ</oboInOwl:hasOBONamespace>
        <oboInOwl:id>GAZ:00193795</oboInOwl:id>
        <rdfs:label>Qa&apos;a Al-Azraq</rdfs:label>
    </owl:NamedIndividual>
    


    <!-- http://purl.obolibrary.org/obo/GAZ_00193797 -->

    <owl:NamedIndividual rdf:about="http://purl.obolibrary.org/obo/GAZ_00193797">
        <obo:RO_0001025 rdf:resource="http://purl.obolibrary.org/obo/GAZ_02000739"/>
        <obo:IAO_0000115>A valley cut into the sandstone and granite rock in southwest Jordan.</obo:IAO_0000115>
        <oboInOwl:hasOBONamespace>GAZ</oboInOwl:hasOBONamespace>
        <oboInOwl:id>GAZ:00193797</oboInOwl:id>
        <rdfs:label>Wadi Rum</rdfs:label>
    </owl:NamedIndividual>
    


    <!-- http://purl.obolibrary.org/obo/GAZ_00193798 -->

    <owl:NamedIndividual rdf:about="http://purl.obolibrary.org/obo/GAZ_00193798">
        <obo:RO_0001025 rdf:resource="http://purl.obolibrary.org/obo/GAZ_02000744"/>
        <obo:IAO_0000115>A wadi in western Jordan.</obo:IAO_0000115>
        <oboInOwl:hasOBONamespace>GAZ</oboInOwl:hasOBONamespace>
        <oboInOwl:id>GAZ:00193798</oboInOwl:id>
        <rdfs:label>Wadi Zered</rdfs:label>
    </owl:NamedIndividual>
    


    <!-- http://purl.obolibrary.org/obo/GAZ_00193804 -->

    <owl:NamedIndividual rdf:about="http://purl.obolibrary.org/obo/GAZ_00193804">
        <obo:RO_0001025 rdf:resource="http://purl.obolibrary.org/obo/GAZ_00007862"/>
        <obo:IAO_0000115>A protected area located on the Red Sea south of Eilat.</obo:IAO_0000115>
        <oboInOwl:hasOBONamespace>GAZ</oboInOwl:hasOBONamespace>
        <oboInOwl:id>GAZ:00193804</oboInOwl:id>
        <rdfs:label>Coral Beach Nature Reserve</rdfs:label>
    </owl:NamedIndividual>
    


    <!-- http://purl.obolibrary.org/obo/GAZ_00193854 -->

    <owl:NamedIndividual rdf:about="http://purl.obolibrary.org/obo/GAZ_00193854">
        <obo:RO_0001025 rdf:resource="http://purl.obolibrary.org/obo/GAZ_00010533"/>
        <obo:IAO_0000115>A protected area. An archeological site. A World Heritage Site.</obo:IAO_0000115>
        <oboInOwl:hasOBONamespace>GAZ</oboInOwl:hasOBONamespace>
        <oboInOwl:id>GAZ:00193854</oboInOwl:id>
        <rdfs:label>Megiddo National Park</rdfs:label>
    </owl:NamedIndividual>
    


    <!-- http://purl.obolibrary.org/obo/GAZ_00193855 -->

    <owl:NamedIndividual rdf:about="http://purl.obolibrary.org/obo/GAZ_00193855">
        <obo:RO_0001025 rdf:resource="http://purl.obolibrary.org/obo/GAZ_00010533"/>
        <obo:IAO_0000115>A protected area. An archeological site.</obo:IAO_0000115>
        <oboInOwl:hasOBONamespace>GAZ</oboInOwl:hasOBONamespace>
        <oboInOwl:id>GAZ:00193855</oboInOwl:id>
        <rdfs:label>Ma&apos;ayan Harod National Park</rdfs:label>
    </owl:NamedIndividual>
    


    <!-- http://purl.obolibrary.org/obo/GAZ_00193856 -->

    <owl:NamedIndividual rdf:about="http://purl.obolibrary.org/obo/GAZ_00193856">
        <obo:RO_0001025 rdf:resource="http://purl.obolibrary.org/obo/GAZ_00193855"/>
        <obo:IAO_0000115>A spring. It emerges from a rocky cave on the slope of Mount Gilboa.</obo:IAO_0000115>
        <oboInOwl:hasOBONamespace>GAZ</oboInOwl:hasOBONamespace>
        <oboInOwl:id>GAZ:00193856</oboInOwl:id>
        <rdfs:label>Ma&apos;ayan Harod</rdfs:label>
    </owl:NamedIndividual>
    


    <!-- http://purl.obolibrary.org/obo/GAZ_00193866 -->

    <owl:NamedIndividual rdf:about="http://purl.obolibrary.org/obo/GAZ_00193866">
        <obo:RO_0001025 rdf:resource="http://purl.obolibrary.org/obo/GAZ_00044915"/>
        <obo:IAO_0000115>A protected area. An archeological site.</obo:IAO_0000115>
        <oboInOwl:hasOBONamespace>GAZ</oboInOwl:hasOBONamespace>
        <oboInOwl:id>GAZ:00193866</oboInOwl:id>
        <rdfs:label>Bet She&apos;an National Park</rdfs:label>
    </owl:NamedIndividual>
    


    <!-- http://purl.obolibrary.org/obo/GAZ_00193868 -->

    <owl:NamedIndividual rdf:about="http://purl.obolibrary.org/obo/GAZ_00193868">
        <obo:IAO_0000115>A protected area located in the central Golan Heights.</obo:IAO_0000115>
        <oboInOwl:hasOBONamespace>GAZ</oboInOwl:hasOBONamespace>
        <oboInOwl:id>GAZ:00193868</oboInOwl:id>
        <rdfs:label>Yehudiya Forest Nature Reserve</rdfs:label>
    </owl:NamedIndividual>
    


    <!-- http://purl.obolibrary.org/obo/GAZ_00193869 -->

    <owl:NamedIndividual rdf:about="http://purl.obolibrary.org/obo/GAZ_00193869">
        <obo:RO_0001025 rdf:resource="http://purl.obolibrary.org/obo/GAZ_00193868"/>
        <obo:IAO_0000115>A river.</obo:IAO_0000115>
        <oboInOwl:hasOBONamespace>GAZ</oboInOwl:hasOBONamespace>
        <oboInOwl:id>GAZ:00193869</oboInOwl:id>
        <rdfs:label>Meshushim Stream</rdfs:label>
    </owl:NamedIndividual>
    


    <!-- http://purl.obolibrary.org/obo/GAZ_00193870 -->

    <owl:NamedIndividual rdf:about="http://purl.obolibrary.org/obo/GAZ_00193870">
        <obo:RO_0001025 rdf:resource="http://purl.obolibrary.org/obo/GAZ_00193868"/>
        <obo:IAO_0000115>A river.</obo:IAO_0000115>
        <oboInOwl:hasOBONamespace>GAZ</oboInOwl:hasOBONamespace>
        <oboInOwl:id>GAZ:00193870</oboInOwl:id>
        <rdfs:label>Yehudiya Stream</rdfs:label>
    </owl:NamedIndividual>
    


    <!-- http://purl.obolibrary.org/obo/GAZ_00193871 -->

    <owl:NamedIndividual rdf:about="http://purl.obolibrary.org/obo/GAZ_00193871">
        <obo:RO_0001025 rdf:resource="http://purl.obolibrary.org/obo/GAZ_00193868"/>
        <obo:IAO_0000115>A river.</obo:IAO_0000115>
        <oboInOwl:hasOBONamespace>GAZ</oboInOwl:hasOBONamespace>
        <oboInOwl:id>GAZ:00193871</oboInOwl:id>
        <rdfs:label>Gamla Stream</rdfs:label>
    </owl:NamedIndividual>
    


    <!-- http://purl.obolibrary.org/obo/GAZ_00193872 -->

    <owl:NamedIndividual rdf:about="http://purl.obolibrary.org/obo/GAZ_00193872">
        <obo:RO_0001025 rdf:resource="http://purl.obolibrary.org/obo/GAZ_00193868"/>
        <obo:IAO_0000115>A river.</obo:IAO_0000115>
        <oboInOwl:hasOBONamespace>GAZ</oboInOwl:hasOBONamespace>
        <oboInOwl:id>GAZ:00193872</oboInOwl:id>
        <rdfs:label>Zavitan Stream</rdfs:label>
    </owl:NamedIndividual>
    


    <!-- http://purl.obolibrary.org/obo/GAZ_00193873 -->

    <owl:NamedIndividual rdf:about="http://purl.obolibrary.org/obo/GAZ_00193873">
        <obo:RO_0001025 rdf:resource="http://purl.obolibrary.org/obo/GAZ_00193868"/>
        <obo:IAO_0000115>A river.</obo:IAO_0000115>
        <oboInOwl:hasOBONamespace>GAZ</oboInOwl:hasOBONamespace>
        <oboInOwl:id>GAZ:00193873</oboInOwl:id>
        <rdfs:label>Daliyot Stream</rdfs:label>
    </owl:NamedIndividual>
    


    <!-- http://purl.obolibrary.org/obo/GAZ_00193876 -->

    <owl:NamedIndividual rdf:about="http://purl.obolibrary.org/obo/GAZ_00193876">
        <obo:RO_0001025 rdf:resource="http://purl.obolibrary.org/obo/GAZ_00193868"/>
        <obo:IAO_0000115>A protected area.</obo:IAO_0000115>
        <oboInOwl:hasOBONamespace>GAZ</oboInOwl:hasOBONamespace>
        <oboInOwl:id>GAZ:00193876</oboInOwl:id>
        <rdfs:label>Meshushim Reserve</rdfs:label>
    </owl:NamedIndividual>
    


    <!-- http://purl.obolibrary.org/obo/GAZ_00193877 -->

    <owl:NamedIndividual rdf:about="http://purl.obolibrary.org/obo/GAZ_00193877">
        <obo:RO_0001025 rdf:resource="http://purl.obolibrary.org/obo/GAZ_00193876"/>
        <obo:IAO_0000115>A lake.</obo:IAO_0000115>
        <oboInOwl:hasOBONamespace>GAZ</oboInOwl:hasOBONamespace>
        <oboInOwl:id>GAZ:00193877</oboInOwl:id>
        <rdfs:label>Meshushim Pool</rdfs:label>
    </owl:NamedIndividual>
    


    <!-- http://purl.obolibrary.org/obo/GAZ_00193883 -->

    <owl:NamedIndividual rdf:about="http://purl.obolibrary.org/obo/GAZ_00193883">
        <obo:IAO_0000115>An Israeili protected area. An archeological site. Located on the slopes of Mount Hermon above the Banias Spring.</obo:IAO_0000115>
        <oboInOwl:hasOBONamespace>GAZ</oboInOwl:hasOBONamespace>
        <oboInOwl:id>GAZ:00193883</oboInOwl:id>
        <rdfs:label>Nimrod Fortress National Park</rdfs:label>
    </owl:NamedIndividual>
    


    <!-- http://purl.obolibrary.org/obo/GAZ_00193885 -->

    <owl:NamedIndividual rdf:about="http://purl.obolibrary.org/obo/GAZ_00193885">
        <obo:RO_0001025 rdf:resource="http://purl.obolibrary.org/obo/GAZ_00008742"/>
        <obo:IAO_0000115>A protected area.</obo:IAO_0000115>
        <oboInOwl:hasOBONamespace>GAZ</oboInOwl:hasOBONamespace>
        <oboInOwl:id>GAZ:00193885</oboInOwl:id>
        <rdfs:label>Hurshat Tal National Park</rdfs:label>
    </owl:NamedIndividual>
    


    <!-- http://purl.obolibrary.org/obo/GAZ_00193886 -->

    <owl:NamedIndividual rdf:about="http://purl.obolibrary.org/obo/GAZ_00193886">
        <obo:RO_0001025 rdf:resource="http://purl.obolibrary.org/obo/GAZ_00008742"/>
        <obo:IAO_0000115>A protected area.</obo:IAO_0000115>
        <oboInOwl:hasOBONamespace>GAZ</oboInOwl:hasOBONamespace>
        <oboInOwl:id>GAZ:00193886</oboInOwl:id>
        <rdfs:label>Hula Nature Reserve</rdfs:label>
    </owl:NamedIndividual>
    


    <!-- http://purl.obolibrary.org/obo/GAZ_00193891 -->

    <owl:NamedIndividual rdf:about="http://purl.obolibrary.org/obo/GAZ_00193891">
        <obo:IAO_0000115>A protected area located in the central Golan Heights.</obo:IAO_0000115>
        <oboInOwl:hasOBONamespace>GAZ</oboInOwl:hasOBONamespace>
        <oboInOwl:id>GAZ:00193891</oboInOwl:id>
        <rdfs:label>Gamla Nature Reserve</rdfs:label>
    </owl:NamedIndividual>
    


    <!-- http://purl.obolibrary.org/obo/GAZ_00193937 -->

    <owl:NamedIndividual rdf:about="http://purl.obolibrary.org/obo/GAZ_00193937">
        <obo:IAO_0000115>A crater lake (maar) in the northeastern Golan Heights, near Mount Hermon. The only sources of the lake are rain water and an underground spring.</obo:IAO_0000115>
        <oboInOwl:hasOBONamespace>GAZ</oboInOwl:hasOBONamespace>
        <oboInOwl:id>GAZ:00193937</oboInOwl:id>
        <rdfs:label>Birkat Ram</rdfs:label>
    </owl:NamedIndividual>
    


    <!-- http://purl.obolibrary.org/obo/GAZ_00193951 -->

    <owl:NamedIndividual rdf:about="http://purl.obolibrary.org/obo/GAZ_00193951">
        <obo:RO_0001025 rdf:resource="http://purl.obolibrary.org/obo/GAZ_00044915"/>
        <obo:IAO_0000115>A large spit of land which now separates the North and the South basins of the Dead Sea. Entirely located in Jordan.</obo:IAO_0000115>
        <oboInOwl:hasOBONamespace>GAZ</oboInOwl:hasOBONamespace>
        <oboInOwl:id>GAZ:00193951</oboInOwl:id>
        <rdfs:label>Lisan Peninsula</rdfs:label>
    </owl:NamedIndividual>
    


    <!-- http://purl.obolibrary.org/obo/GAZ_00251586 -->

    <owl:NamedIndividual rdf:about="http://purl.obolibrary.org/obo/GAZ_00251586">
        <obo:RO_0001025 rdf:resource="http://purl.obolibrary.org/obo/GAZ_02000743"/>
        <obo:IAO_0000115>A river that rises in the hills southwest of Irbid city and drains west into the Jordan Valley, entering the Jordan River about 20 km south of Lake Tiberias.</obo:IAO_0000115>
        <oboInOwl:hasOBONamespace>GAZ</oboInOwl:hasOBONamespace>
        <oboInOwl:id>GAZ:00251586</oboInOwl:id>
        <rdfs:label>Wadi Ziglab</rdfs:label>
    </owl:NamedIndividual>
    


    <!-- http://purl.obolibrary.org/obo/GAZ_00251587 -->

    <owl:NamedIndividual rdf:about="http://purl.obolibrary.org/obo/GAZ_00251587">
        <obo:IAO_0000115>A dam. Located about 15 km south-southwest of Ajlun.</obo:IAO_0000115>
        <oboInOwl:hasOBONamespace>GAZ</oboInOwl:hasOBONamespace>
        <oboInOwl:id>GAZ:00251587</oboInOwl:id>
        <rdfs:label>KingTalal Dam</rdfs:label>
    </owl:NamedIndividual>
    


    <!-- http://purl.obolibrary.org/obo/GAZ_00251588 -->

    <owl:NamedIndividual rdf:about="http://purl.obolibrary.org/obo/GAZ_00251588">
        <obo:RO_0001025 rdf:resource="http://purl.obolibrary.org/obo/GAZ_02000748"/>
        <obo:IAO_0000115>The main sewage treatment plant for the city of Amman; it comprises a large area of open, manmade pools in a broad depression close to Wadi Dhulayl, a tributary of the Zarqa River.</obo:IAO_0000115>
        <oboInOwl:hasOBONamespace>GAZ</oboInOwl:hasOBONamespace>
        <oboInOwl:id>GAZ:00251588</oboInOwl:id>
        <rdfs:label>Kherbit Al-Samra Sewage Treatment Plant</rdfs:label>
    </owl:NamedIndividual>
    


    <!-- http://purl.obolibrary.org/obo/GAZ_00251592 -->

    <owl:NamedIndividual rdf:about="http://purl.obolibrary.org/obo/GAZ_00251592">
        <obo:IAO_0000115>A dam.</obo:IAO_0000115>
        <oboInOwl:hasOBONamespace>GAZ</oboInOwl:hasOBONamespace>
        <oboInOwl:id>GAZ:00251592</oboInOwl:id>
        <rdfs:label>Kafrein Dam</rdfs:label>
    </owl:NamedIndividual>
    


    <!-- http://purl.obolibrary.org/obo/GAZ_00251593 -->

    <owl:NamedIndividual rdf:about="http://purl.obolibrary.org/obo/GAZ_00251593">
        <obo:IAO_0000115>A dam.</obo:IAO_0000115>
        <oboInOwl:hasOBONamespace>GAZ</oboInOwl:hasOBONamespace>
        <oboInOwl:id>GAZ:00251593</oboInOwl:id>
        <rdfs:label>Shu&apos;eib Dam</rdfs:label>
    </owl:NamedIndividual>
    


    <!-- http://purl.obolibrary.org/obo/GAZ_00251594 -->

    <owl:NamedIndividual rdf:about="http://purl.obolibrary.org/obo/GAZ_00251594">
        <obo:RO_0001025 rdf:resource="http://purl.obolibrary.org/obo/GAZ_00044915"/>
        <obo:IAO_0000115>A saline lake.</obo:IAO_0000115>
        <oboInOwl:hasOBONamespace>GAZ</oboInOwl:hasOBONamespace>
        <oboInOwl:id>GAZ:00251594</oboInOwl:id>
        <rdfs:label>Kibed Pool</rdfs:label>
    </owl:NamedIndividual>
    


    <!-- http://purl.obolibrary.org/obo/GAZ_00251595 -->

    <owl:NamedIndividual rdf:about="http://purl.obolibrary.org/obo/GAZ_00251595">
        <obo:IAO_0000115>A wadi. It enters Wadi Mujib from the north only a few km from the shores of the Dead Sea.</obo:IAO_0000115>
        <oboInOwl:hasOBONamespace>GAZ</oboInOwl:hasOBONamespace>
        <oboInOwl:id>GAZ:00251595</oboInOwl:id>
        <rdfs:label>Wadi Hidan</rdfs:label>
    </owl:NamedIndividual>
    


    <!-- http://purl.obolibrary.org/obo/GAZ_00251596 -->

    <owl:NamedIndividual rdf:about="http://purl.obolibrary.org/obo/GAZ_00251596">
        <obo:RO_0001025 rdf:resource="http://purl.obolibrary.org/obo/GAZ_02000740"/>
        <obo:IAO_0000115>A freshwater lake. Located in the Eastern Desert, 12 km north-northwest of the village of Muqat on the main Amman to Baghdad road, about 200 km east-northeast of Amman, Mafraq Governorate.</obo:IAO_0000115>
        <oboInOwl:hasOBONamespace>GAZ</oboInOwl:hasOBONamespace>
        <oboInOwl:id>GAZ:00251596</oboInOwl:id>
        <rdfs:label>Ghadir Burqu</rdfs:label>
    </owl:NamedIndividual>
    


    <!-- http://purl.obolibrary.org/obo/GAZ_00251597 -->

    <owl:NamedIndividual rdf:about="http://purl.obolibrary.org/obo/GAZ_00251597">
        <obo:RO_0001025 rdf:resource="http://purl.obolibrary.org/obo/GAZ_02000748"/>
        <obo:IAO_0000115>A seasonal playa lake. Located in the Eastern Desert, 7 km north of the main Zarqa to Azraq highway, about 40 km east of Zarqa and 60 km east-northeast of Amman, Zarqa Governorate.</obo:IAO_0000115>
        <oboInOwl:hasOBONamespace>GAZ</oboInOwl:hasOBONamespace>
        <oboInOwl:id>GAZ:00251597</oboInOwl:id>
        <rdfs:label>Qa Khana</rdfs:label>
    </owl:NamedIndividual>
    


    <!-- http://purl.obolibrary.org/obo/GAZ_00251598 -->

    <owl:NamedIndividual rdf:about="http://purl.obolibrary.org/obo/GAZ_00251598">
        <obo:RO_0001025 rdf:resource="http://purl.obolibrary.org/obo/GAZ_00193794"/>
        <obo:IAO_0000115>An oasis. Located in the Eastern Desert, about 85 km east southeast of Amman, Zarqa Governorate.</obo:IAO_0000115>
        <oboInOwl:hasOBONamespace>GAZ</oboInOwl:hasOBONamespace>
        <oboInOwl:id>GAZ:00251598</oboInOwl:id>
        <rdfs:label>Azraq Oasis</rdfs:label>
    </owl:NamedIndividual>
    


    <!-- http://purl.obolibrary.org/obo/GAZ_00251600 -->

    <owl:NamedIndividual rdf:about="http://purl.obolibrary.org/obo/GAZ_00251600">
        <obo:RO_0001025 rdf:resource="http://purl.obolibrary.org/obo/GAZ_02000739"/>
        <obo:IAO_0000115>A seasonal playa wetland. Located in the Eastern Desert, about 45 km east of Ma&apos;an, Ma&apos;an Governorate.</obo:IAO_0000115>
        <oboInOwl:hasOBONamespace>GAZ</oboInOwl:hasOBONamespace>
        <oboInOwl:id>GAZ:00251600</oboInOwl:id>
        <rdfs:label>Qa Al Jafr</rdfs:label>
    </owl:NamedIndividual>
    


    <!-- http://purl.obolibrary.org/obo/GAZ_00251601 -->

    <owl:NamedIndividual rdf:about="http://purl.obolibrary.org/obo/GAZ_00251601">
        <obo:RO_0001025 rdf:resource="http://purl.obolibrary.org/obo/GAZ_02000739"/>
        <obo:IAO_0000115>A playa wetland. Located in the Eastern Desert about 10 km east of Wadi Rum and 50 km east-northeast of Aqaba, Ma&apos;an Governorate.</obo:IAO_0000115>
        <oboInOwl:hasOBONamespace>GAZ</oboInOwl:hasOBONamespace>
        <oboInOwl:id>GAZ:00251601</oboInOwl:id>
        <rdfs:label>Qa Disi</rdfs:label>
    </owl:NamedIndividual>
    


    <!-- http://purl.obolibrary.org/obo/GAZ_00256566 -->

    <owl:NamedIndividual rdf:about="http://purl.obolibrary.org/obo/GAZ_00256566">
        <obo:IAO_0000115>A seasonally flooded saline lake in the Syrian Desert. Located several km south and southeast of Tadmur (Palmyra), Homs Governorate.</obo:IAO_0000115>
        <oboInOwl:hasOBONamespace>GAZ</oboInOwl:hasOBONamespace>
        <oboInOwl:id>GAZ:00256566</oboInOwl:id>
        <rdfs:label>Sabkhat Muh</rdfs:label>
    </owl:NamedIndividual>
    


    <!-- http://purl.obolibrary.org/obo/GAZ_02000738 -->

    <owl:NamedIndividual rdf:about="http://purl.obolibrary.org/obo/GAZ_02000738"/>
    


    <!-- http://purl.obolibrary.org/obo/GAZ_02000739 -->

    <owl:NamedIndividual rdf:about="http://purl.obolibrary.org/obo/GAZ_02000739"/>
    


    <!-- http://purl.obolibrary.org/obo/GAZ_02000740 -->

    <owl:NamedIndividual rdf:about="http://purl.obolibrary.org/obo/GAZ_02000740"/>
    


    <!-- http://purl.obolibrary.org/obo/GAZ_02000741 -->

    <owl:NamedIndividual rdf:about="http://purl.obolibrary.org/obo/GAZ_02000741"/>
    


    <!-- http://purl.obolibrary.org/obo/GAZ_02000742 -->

    <owl:NamedIndividual rdf:about="http://purl.obolibrary.org/obo/GAZ_02000742"/>
    


    <!-- http://purl.obolibrary.org/obo/GAZ_02000743 -->

    <owl:NamedIndividual rdf:about="http://purl.obolibrary.org/obo/GAZ_02000743"/>
    


    <!-- http://purl.obolibrary.org/obo/GAZ_02000744 -->

    <owl:NamedIndividual rdf:about="http://purl.obolibrary.org/obo/GAZ_02000744"/>
    


    <!-- http://purl.obolibrary.org/obo/GAZ_02000745 -->

    <owl:NamedIndividual rdf:about="http://purl.obolibrary.org/obo/GAZ_02000745"/>
    


    <!-- http://purl.obolibrary.org/obo/GAZ_02000746 -->

    <owl:NamedIndividual rdf:about="http://purl.obolibrary.org/obo/GAZ_02000746"/>
    


    <!-- http://purl.obolibrary.org/obo/GAZ_02000747 -->

    <owl:NamedIndividual rdf:about="http://purl.obolibrary.org/obo/GAZ_02000747"/>
    


    <!-- http://purl.obolibrary.org/obo/GAZ_02000748 -->

    <owl:NamedIndividual rdf:about="http://purl.obolibrary.org/obo/GAZ_02000748"/>
    


    <!-- http://purl.obolibrary.org/obo/GAZ_02000749 -->

    <owl:NamedIndividual rdf:about="http://purl.obolibrary.org/obo/GAZ_02000749"/>
    


    <!-- 
    ///////////////////////////////////////////////////////////////////////////////////////
    //
    // Annotations
    //
    ///////////////////////////////////////////////////////////////////////////////////////
     -->

    <rdf:Description rdf:about="http://purl.obolibrary.org/obo/GAZ_00009510">
        <rdfs:label>Governorate (Jordan)</rdfs:label>
        <oboInOwl:hasOBONamespace>GAZ</oboInOwl:hasOBONamespace>
        <oboInOwl:id>GAZ:00009510</oboInOwl:id>
    </rdf:Description>
    <rdf:Description rdf:about="http://purl.obolibrary.org/obo/GAZ_02000738">
        <oboInOwl:hasOBONamespace>GAZ</oboInOwl:hasOBONamespace>
        <rdfs:label>Governorate of Jerash</rdfs:label>
        <oboInOwl:id>GAZ:02000738</oboInOwl:id>
        <obo:IAO_0000115>One of the governorates of Jordan; it is located north of Amman, Jordan&apos;s capital.</obo:IAO_0000115>
    </rdf:Description>
    <rdf:Description rdf:about="http://purl.obolibrary.org/obo/GAZ_02000739">
        <oboInOwl:hasOBONamespace>GAZ</oboInOwl:hasOBONamespace>
        <rdfs:label>Governorate of Ma&apos;an</rdfs:label>
        <obo:IAO_0000115>One of the governorates of Jordan, it is located south of Amman, Jordan&apos;s capital. Its capital is the city of Ma&apos;an.</obo:IAO_0000115>
        <oboInOwl:id>GAZ:02000739</oboInOwl:id>
    </rdf:Description>
    <rdf:Description rdf:about="http://purl.obolibrary.org/obo/GAZ_02000740">
        <oboInOwl:hasOBONamespace>GAZ</oboInOwl:hasOBONamespace>
        <obo:IAO_0000115>One of the governorates of Jordan, located to the north-east of Amman, capital of Jordan.</obo:IAO_0000115>
        <rdfs:label>Governorate of Mafraq</rdfs:label>
        <oboInOwl:id>GAZ:02000740</oboInOwl:id>
    </rdf:Description>
    <rdf:Description rdf:about="http://purl.obolibrary.org/obo/GAZ_02000741">
        <oboInOwl:id>GAZ:02000741</oboInOwl:id>
        <oboInOwl:hasOBONamespace>GAZ</oboInOwl:hasOBONamespace>
        <obo:IAO_0000115>One of the governorates of Jordan, it is located west of Amman, capital of Jordan. Its capital is Madaba.</obo:IAO_0000115>
        <rdfs:label>Governorate of Madaba</rdfs:label>
    </rdf:Description>
    <rdf:Description rdf:about="http://purl.obolibrary.org/obo/GAZ_02000742">
        <rdfs:label>Governorate of Balqa</rdfs:label>
        <oboInOwl:id>GAZ:02000742</oboInOwl:id>
        <oboInOwl:hasOBONamespace>GAZ</oboInOwl:hasOBONamespace>
        <obo:IAO_0000115>One of the governorates of Jordan. It is located northwest of Amman, Jordan&apos;s capital.</obo:IAO_0000115>
    </rdf:Description>
    <rdf:Description rdf:about="http://purl.obolibrary.org/obo/GAZ_02000743">
        <oboInOwl:id>GAZ:02000743</oboInOwl:id>
        <oboInOwl:hasOBONamespace>GAZ</oboInOwl:hasOBONamespace>
        <rdfs:label>Governorate of Irbid</rdfs:label>
        <obo:IAO_0000115>One of the governorates of Jordan. It is located north of Amman, Jordan&apos;s capital. The center of the governorate of Irbid is the city of Irbid.</obo:IAO_0000115>
    </rdf:Description>
    <rdf:Description rdf:about="http://purl.obolibrary.org/obo/GAZ_02000744">
        <obo:IAO_0000115>One of the governorates of Jordan, located south-west of Amman, Jordan&apos;s capital. Its capital is Al Karak.</obo:IAO_0000115>
        <oboInOwl:id>GAZ:02000744</oboInOwl:id>
        <oboInOwl:hasOBONamespace>GAZ</oboInOwl:hasOBONamespace>
        <rdfs:label>Governorate of Karak</rdfs:label>
    </rdf:Description>
    <rdf:Description rdf:about="http://purl.obolibrary.org/obo/GAZ_02000745">
        <obo:IAO_0000115>One of the governorates of Jordan, located south of Amman, capital of Jordan. Its capital is Aqaba.</obo:IAO_0000115>
        <oboInOwl:id>GAZ:02000745</oboInOwl:id>
        <oboInOwl:hasOBONamespace>GAZ</oboInOwl:hasOBONamespace>
        <rdfs:label>Governorate of Aqaba</rdfs:label>
    </rdf:Description>
    <rdf:Description rdf:about="http://purl.obolibrary.org/obo/GAZ_02000746">
        <oboInOwl:hasOBONamespace>GAZ</oboInOwl:hasOBONamespace>
        <oboInOwl:id>GAZ:02000746</oboInOwl:id>
        <obo:IAO_0000115>One of the governorates of Jordan, located north of Amman the capital of Jordan.</obo:IAO_0000115>
        <rdfs:label>Governorate of Ajlun</rdfs:label>
    </rdf:Description>
    <rdf:Description rdf:about="http://purl.obolibrary.org/obo/GAZ_02000747">
        <oboInOwl:hasOBONamespace>GAZ</oboInOwl:hasOBONamespace>
        <oboInOwl:id>GAZ:02000747</oboInOwl:id>
        <obo:IAO_0000115>One of the governorates of Jordan. This governorate&apos;s capital is the City of Amman, which is Jordan&apos;s capital as well.</obo:IAO_0000115>
        <rdfs:label>Governorate of Amman</rdfs:label>
    </rdf:Description>
    <rdf:Description rdf:about="http://purl.obolibrary.org/obo/GAZ_02000748">
        <oboInOwl:hasOBONamespace>GAZ</oboInOwl:hasOBONamespace>
        <rdfs:label>Governorate of Zarqa</rdfs:label>
        <obo:IAO_0000115>One of the governorates of Jordan, located east of Amman, the capital of Jordan. Its capital is Zarqa.</obo:IAO_0000115>
        <oboInOwl:id>GAZ:02000748</oboInOwl:id>
    </rdf:Description>
    <rdf:Description rdf:about="http://purl.obolibrary.org/obo/GAZ_02000749">
        <oboInOwl:hasOBONamespace>GAZ</oboInOwl:hasOBONamespace>
        <rdfs:label>Governorate of Tafilah</rdfs:label>
        <obo:IAO_0000115>One of the governorates of Jordan, located south-west of Amman, Jordan&apos;s capital.</obo:IAO_0000115>
        <oboInOwl:id>GAZ:02000749</oboInOwl:id>
    </rdf:Description>
</rdf:RDF>



<!-- Generated by the OWL API (version 4.5.6) https://github.com/owlcs/owlapi -->

