<?xml version="1.0"?>
<rdf:RDF xmlns="http://purl.obolibrary.org/obo/gaz/subsets/countries/Kyrgyzstan.owl#"
     xml:base="http://purl.obolibrary.org/obo/gaz/subsets/countries/Kyrgyzstan.owl"
     xmlns:dc="http://purl.org/dc/elements/1.1/"
     xmlns:obo="http://purl.obolibrary.org/obo/"
     xmlns:owl="http://www.w3.org/2002/07/owl#"
     xmlns:rdf="http://www.w3.org/1999/02/22-rdf-syntax-ns#"
     xmlns:xml="http://www.w3.org/XML/1998/namespace"
     xmlns:xsd="http://www.w3.org/2001/XMLSchema#"
     xmlns:envo="http://purl.obolibrary.org/obo/envo#"
     xmlns:rdfs="http://www.w3.org/2000/01/rdf-schema#"
     xmlns:oboInOwl="http://www.geneontology.org/formats/oboInOwl#">
    <owl:Ontology rdf:about="http://purl.obolibrary.org/obo/gaz/subsets/countries/Kyrgyzstan.owl">
        <owl:imports rdf:resource="http://purl.obolibrary.org/obo/gaz/imports/envo_import.owl"/>
        <owl:imports rdf:resource="http://purl.obolibrary.org/obo/gaz/imports/ro_import.owl"/>
    </owl:Ontology>
    


    <!-- 
    ///////////////////////////////////////////////////////////////////////////////////////
    //
    // Annotation properties
    //
    ///////////////////////////////////////////////////////////////////////////////////////
     -->

    


    <!-- http://purl.obolibrary.org/obo/IAO_0000115 -->

    <owl:AnnotationProperty rdf:about="http://purl.obolibrary.org/obo/IAO_0000115"/>
    


    <!-- http://www.geneontology.org/formats/oboInOwl#hasOBONamespace -->

    <owl:AnnotationProperty rdf:about="http://www.geneontology.org/formats/oboInOwl#hasOBONamespace"/>
    


    <!-- http://www.geneontology.org/formats/oboInOwl#id -->

    <owl:AnnotationProperty rdf:about="http://www.geneontology.org/formats/oboInOwl#id"/>
    


    <!-- 
    ///////////////////////////////////////////////////////////////////////////////////////
    //
    // Object Properties
    //
    ///////////////////////////////////////////////////////////////////////////////////////
     -->

    


    <!-- http://purl.obolibrary.org/obo/RO_0001025 -->

    <owl:ObjectProperty rdf:about="http://purl.obolibrary.org/obo/RO_0001025"/>
    


    <!-- 
    ///////////////////////////////////////////////////////////////////////////////////////
    //
    // Classes
    //
    ///////////////////////////////////////////////////////////////////////////////////////
     -->

    


    <!-- http://purl.obolibrary.org/obo/ENVO_00000009 -->

    <owl:Class rdf:about="http://purl.obolibrary.org/obo/ENVO_00000009"/>
    


    <!-- http://purl.obolibrary.org/obo/ENVO_00000020 -->

    <owl:Class rdf:about="http://purl.obolibrary.org/obo/ENVO_00000020"/>
    


    <!-- http://purl.obolibrary.org/obo/GAZ_00009463 -->

    <owl:Class rdf:about="http://purl.obolibrary.org/obo/GAZ_00009463"/>
    


    <!-- http://purl.obolibrary.org/obo/GAZ_00022023 -->

    <owl:Class rdf:about="http://purl.obolibrary.org/obo/GAZ_00022023">
        <rdfs:subClassOf rdf:resource="http://purl.obolibrary.org/obo/GAZ_02000779"/>
        <oboInOwl:hasOBONamespace>GAZ</oboInOwl:hasOBONamespace>
        <oboInOwl:id>GAZ:00022023</oboInOwl:id>
        <rdfs:label>Osh City</rdfs:label>
    </owl:Class>
    


    <!-- http://purl.obolibrary.org/obo/GAZ_02000771 -->

    <owl:Class rdf:about="http://purl.obolibrary.org/obo/GAZ_02000771">
        <rdfs:subClassOf rdf:resource="http://purl.obolibrary.org/obo/GAZ_00009463"/>
    </owl:Class>
    


    <!-- http://purl.obolibrary.org/obo/GAZ_02000772 -->

    <owl:Class rdf:about="http://purl.obolibrary.org/obo/GAZ_02000772">
        <rdfs:subClassOf rdf:resource="http://purl.obolibrary.org/obo/GAZ_00009463"/>
    </owl:Class>
    


    <!-- http://purl.obolibrary.org/obo/GAZ_02000773 -->

    <owl:Class rdf:about="http://purl.obolibrary.org/obo/GAZ_02000773">
        <rdfs:subClassOf rdf:resource="http://purl.obolibrary.org/obo/GAZ_00009463"/>
    </owl:Class>
    


    <!-- http://purl.obolibrary.org/obo/GAZ_02000774 -->

    <owl:Class rdf:about="http://purl.obolibrary.org/obo/GAZ_02000774">
        <rdfs:subClassOf rdf:resource="http://purl.obolibrary.org/obo/GAZ_02000779"/>
    </owl:Class>
    


    <!-- http://purl.obolibrary.org/obo/GAZ_02000775 -->

    <owl:Class rdf:about="http://purl.obolibrary.org/obo/GAZ_02000775">
        <rdfs:subClassOf rdf:resource="http://purl.obolibrary.org/obo/GAZ_00009463"/>
    </owl:Class>
    


    <!-- http://purl.obolibrary.org/obo/GAZ_02000776 -->

    <owl:Class rdf:about="http://purl.obolibrary.org/obo/GAZ_02000776">
        <rdfs:subClassOf rdf:resource="http://purl.obolibrary.org/obo/GAZ_00009463"/>
    </owl:Class>
    


    <!-- http://purl.obolibrary.org/obo/GAZ_02000777 -->

    <owl:Class rdf:about="http://purl.obolibrary.org/obo/GAZ_02000777">
        <rdfs:subClassOf rdf:resource="http://purl.obolibrary.org/obo/GAZ_00009463"/>
    </owl:Class>
    


    <!-- http://purl.obolibrary.org/obo/GAZ_02000778 -->

    <owl:Class rdf:about="http://purl.obolibrary.org/obo/GAZ_02000778">
        <rdfs:subClassOf rdf:resource="http://purl.obolibrary.org/obo/GAZ_00009463"/>
    </owl:Class>
    


    <!-- http://purl.obolibrary.org/obo/GAZ_02000779 -->

    <owl:Class rdf:about="http://purl.obolibrary.org/obo/GAZ_02000779"/>
    


    <!-- 
    ///////////////////////////////////////////////////////////////////////////////////////
    //
    // Individuals
    //
    ///////////////////////////////////////////////////////////////////////////////////////
     -->

    


    <!-- http://purl.obolibrary.org/obo/GAZ_00006893 -->

    <owl:NamedIndividual rdf:about="http://purl.obolibrary.org/obo/GAZ_00006893">
        <rdf:type rdf:resource="http://purl.obolibrary.org/obo/ENVO_00000009"/>
        <obo:IAO_0000115>A country in Central Asia. Landlocked and mountainous, it is bordered by Kazakhstan to the north, Uzbekistan to the west, Tajikistan to the southwest and China to the east. Kyrgyzstan is divided into seven provinces (oblast. The capital, Bishkek, and the second large city Osh are administratively the independent cities (shaar) with a status equal to a province. Each province comprises a number of districts (raions).</obo:IAO_0000115>
        <oboInOwl:hasOBONamespace>GAZ</oboInOwl:hasOBONamespace>
        <oboInOwl:id>GAZ:00006893</oboInOwl:id>
        <rdfs:label>Kyrgyzstan</rdfs:label>
    </owl:NamedIndividual>
    


    <!-- http://purl.obolibrary.org/obo/GAZ_00008311 -->

    <owl:NamedIndividual rdf:about="http://purl.obolibrary.org/obo/GAZ_00008311">
        <obo:RO_0001025 rdf:resource="http://purl.obolibrary.org/obo/GAZ_00006893"/>
        <obo:IAO_0000115>A mountain range. It lies to the north and west of the Taklamakan Desert in the border region of Kazakhstan, Kyrgyzstan and the Xinjiang Uyghur Autonomous Region of western China. In the south it links up with the Pamir Mountains. It also extends into the Chinese province of Xinjiang and into the northern areas of Pakistan, where it joins the Hindu Kush. In Western cartography, the eastern end of the Tian Shan is usually understood to be just west of Urumqi, while the range to the east of that city is known as the Bogda Shan. However, in Chinese cartography, from the Han Dynasty to the present, the Tian Shan is also considered to include the Bogda Shan and Barkol ranges. The Tian Shan are a part of the Himalayan orogenic belt which was formed by the collision of the Indian and Eurasian plates in the Cenozoic era. They are one of the longest mountain ranges in Central Asia, stretching some 2,800 km eastward from Tashkent in Uzbekistan.</obo:IAO_0000115>
        <oboInOwl:hasOBONamespace>GAZ</oboInOwl:hasOBONamespace>
        <oboInOwl:id>GAZ:00008311</oboInOwl:id>
        <rdfs:label>Tien Shan</rdfs:label>
    </owl:NamedIndividual>
    


    <!-- http://purl.obolibrary.org/obo/GAZ_00008373 -->

    <owl:NamedIndividual rdf:about="http://purl.obolibrary.org/obo/GAZ_00008373">
        <obo:RO_0001025 rdf:resource="http://purl.obolibrary.org/obo/GAZ_00006893"/>
        <oboInOwl:hasOBONamespace>GAZ</oboInOwl:hasOBONamespace>
        <oboInOwl:id>GAZ:00008373</oboInOwl:id>
        <rdfs:label>Vakhsh Valley</rdfs:label>
    </owl:NamedIndividual>
    


    <!-- http://purl.obolibrary.org/obo/GAZ_00009463 -->

    <owl:NamedIndividual rdf:about="http://purl.obolibrary.org/obo/GAZ_00009463">
        <obo:RO_0001025 rdf:resource="http://purl.obolibrary.org/obo/GAZ_00006893"/>
    </owl:NamedIndividual>
    


    <!-- http://purl.obolibrary.org/obo/GAZ_00021983 -->

    <owl:NamedIndividual rdf:about="http://purl.obolibrary.org/obo/GAZ_00021983">
        <obo:RO_0001025 rdf:resource="http://purl.obolibrary.org/obo/GAZ_02000777"/>
        <oboInOwl:hasOBONamespace>GAZ</oboInOwl:hasOBONamespace>
        <oboInOwl:id>GAZ:00021983</oboInOwl:id>
        <rdfs:label>Batken District</rdfs:label>
    </owl:NamedIndividual>
    


    <!-- http://purl.obolibrary.org/obo/GAZ_00021984 -->

    <owl:NamedIndividual rdf:about="http://purl.obolibrary.org/obo/GAZ_00021984">
        <obo:RO_0001025 rdf:resource="http://purl.obolibrary.org/obo/GAZ_02000777"/>
        <oboInOwl:hasOBONamespace>GAZ</oboInOwl:hasOBONamespace>
        <oboInOwl:id>GAZ:00021984</oboInOwl:id>
        <rdfs:label>Kadamjai District</rdfs:label>
    </owl:NamedIndividual>
    


    <!-- http://purl.obolibrary.org/obo/GAZ_00021985 -->

    <owl:NamedIndividual rdf:about="http://purl.obolibrary.org/obo/GAZ_00021985">
        <obo:RO_0001025 rdf:resource="http://purl.obolibrary.org/obo/GAZ_02000777"/>
        <oboInOwl:hasOBONamespace>GAZ</oboInOwl:hasOBONamespace>
        <oboInOwl:id>GAZ:00021985</oboInOwl:id>
        <rdfs:label>Lailak District</rdfs:label>
    </owl:NamedIndividual>
    


    <!-- http://purl.obolibrary.org/obo/GAZ_00021986 -->

    <owl:NamedIndividual rdf:about="http://purl.obolibrary.org/obo/GAZ_00021986">
        <obo:RO_0001025 rdf:resource="http://purl.obolibrary.org/obo/GAZ_02000774"/>
        <oboInOwl:hasOBONamespace>GAZ</oboInOwl:hasOBONamespace>
        <oboInOwl:id>GAZ:00021986</oboInOwl:id>
        <rdfs:label>Alamudun District</rdfs:label>
    </owl:NamedIndividual>
    


    <!-- http://purl.obolibrary.org/obo/GAZ_00021987 -->

    <owl:NamedIndividual rdf:about="http://purl.obolibrary.org/obo/GAZ_00021987">
        <obo:RO_0001025 rdf:resource="http://purl.obolibrary.org/obo/GAZ_02000775"/>
        <oboInOwl:hasOBONamespace>GAZ</oboInOwl:hasOBONamespace>
        <oboInOwl:id>GAZ:00021987</oboInOwl:id>
        <rdfs:label>At-Bashi District</rdfs:label>
    </owl:NamedIndividual>
    


    <!-- http://purl.obolibrary.org/obo/GAZ_00021988 -->

    <owl:NamedIndividual rdf:about="http://purl.obolibrary.org/obo/GAZ_00021988">
        <obo:RO_0001025 rdf:resource="http://purl.obolibrary.org/obo/GAZ_02000775"/>
        <oboInOwl:hasOBONamespace>GAZ</oboInOwl:hasOBONamespace>
        <oboInOwl:id>GAZ:00021988</oboInOwl:id>
        <rdfs:label>Tien-Shan District</rdfs:label>
    </owl:NamedIndividual>
    


    <!-- http://purl.obolibrary.org/obo/GAZ_00021989 -->

    <owl:NamedIndividual rdf:about="http://purl.obolibrary.org/obo/GAZ_00021989">
        <obo:RO_0001025 rdf:resource="http://purl.obolibrary.org/obo/GAZ_02000772"/>
        <oboInOwl:hasOBONamespace>GAZ</oboInOwl:hasOBONamespace>
        <oboInOwl:id>GAZ:00021989</oboInOwl:id>
        <rdfs:label>Ysyk-Ata District</rdfs:label>
    </owl:NamedIndividual>
    


    <!-- http://purl.obolibrary.org/obo/GAZ_00021990 -->

    <owl:NamedIndividual rdf:about="http://purl.obolibrary.org/obo/GAZ_00021990">
        <obo:RO_0001025 rdf:resource="http://purl.obolibrary.org/obo/GAZ_02000772"/>
        <oboInOwl:hasOBONamespace>GAZ</oboInOwl:hasOBONamespace>
        <oboInOwl:id>GAZ:00021990</oboInOwl:id>
        <rdfs:label>Chui District</rdfs:label>
    </owl:NamedIndividual>
    


    <!-- http://purl.obolibrary.org/obo/GAZ_00021991 -->

    <owl:NamedIndividual rdf:about="http://purl.obolibrary.org/obo/GAZ_00021991">
        <obo:RO_0001025 rdf:resource="http://purl.obolibrary.org/obo/GAZ_02000772"/>
        <oboInOwl:hasOBONamespace>GAZ</oboInOwl:hasOBONamespace>
        <oboInOwl:id>GAZ:00021991</oboInOwl:id>
        <rdfs:label>Sokuluk District</rdfs:label>
    </owl:NamedIndividual>
    


    <!-- http://purl.obolibrary.org/obo/GAZ_00021992 -->

    <owl:NamedIndividual rdf:about="http://purl.obolibrary.org/obo/GAZ_00021992">
        <obo:RO_0001025 rdf:resource="http://purl.obolibrary.org/obo/GAZ_02000772"/>
        <oboInOwl:hasOBONamespace>GAZ</oboInOwl:hasOBONamespace>
        <oboInOwl:id>GAZ:00021992</oboInOwl:id>
        <rdfs:label>Jaiyl District</rdfs:label>
    </owl:NamedIndividual>
    


    <!-- http://purl.obolibrary.org/obo/GAZ_00021993 -->

    <owl:NamedIndividual rdf:about="http://purl.obolibrary.org/obo/GAZ_00021993">
        <obo:RO_0001025 rdf:resource="http://purl.obolibrary.org/obo/GAZ_02000772"/>
        <oboInOwl:hasOBONamespace>GAZ</oboInOwl:hasOBONamespace>
        <oboInOwl:id>GAZ:00021993</oboInOwl:id>
        <rdfs:label>Moskovsky District</rdfs:label>
    </owl:NamedIndividual>
    


    <!-- http://purl.obolibrary.org/obo/GAZ_00021994 -->

    <owl:NamedIndividual rdf:about="http://purl.obolibrary.org/obo/GAZ_00021994">
        <obo:RO_0001025 rdf:resource="http://purl.obolibrary.org/obo/GAZ_02000772"/>
        <oboInOwl:hasOBONamespace>GAZ</oboInOwl:hasOBONamespace>
        <oboInOwl:id>GAZ:00021994</oboInOwl:id>
        <rdfs:label>Kemin District</rdfs:label>
    </owl:NamedIndividual>
    


    <!-- http://purl.obolibrary.org/obo/GAZ_00021995 -->

    <owl:NamedIndividual rdf:about="http://purl.obolibrary.org/obo/GAZ_00021995">
        <obo:RO_0001025 rdf:resource="http://purl.obolibrary.org/obo/GAZ_02000772"/>
        <oboInOwl:hasOBONamespace>GAZ</oboInOwl:hasOBONamespace>
        <oboInOwl:id>GAZ:00021995</oboInOwl:id>
        <rdfs:label>Panfilov District</rdfs:label>
    </owl:NamedIndividual>
    


    <!-- http://purl.obolibrary.org/obo/GAZ_00021996 -->

    <owl:NamedIndividual rdf:about="http://purl.obolibrary.org/obo/GAZ_00021996">
        <obo:RO_0001025 rdf:resource="http://purl.obolibrary.org/obo/GAZ_02000771"/>
        <oboInOwl:hasOBONamespace>GAZ</oboInOwl:hasOBONamespace>
        <oboInOwl:id>GAZ:00021996</oboInOwl:id>
        <rdfs:label>Nooken District</rdfs:label>
    </owl:NamedIndividual>
    


    <!-- http://purl.obolibrary.org/obo/GAZ_00021997 -->

    <owl:NamedIndividual rdf:about="http://purl.obolibrary.org/obo/GAZ_00021997">
        <obo:RO_0001025 rdf:resource="http://purl.obolibrary.org/obo/GAZ_02000778"/>
        <oboInOwl:hasOBONamespace>GAZ</oboInOwl:hasOBONamespace>
        <oboInOwl:id>GAZ:00021997</oboInOwl:id>
        <rdfs:label>Ak-Suu District</rdfs:label>
    </owl:NamedIndividual>
    


    <!-- http://purl.obolibrary.org/obo/GAZ_00021998 -->

    <owl:NamedIndividual rdf:about="http://purl.obolibrary.org/obo/GAZ_00021998">
        <obo:RO_0001025 rdf:resource="http://purl.obolibrary.org/obo/GAZ_02000778"/>
        <oboInOwl:hasOBONamespace>GAZ</oboInOwl:hasOBONamespace>
        <oboInOwl:id>GAZ:00021998</oboInOwl:id>
        <rdfs:label>Djety-Oguz District</rdfs:label>
    </owl:NamedIndividual>
    


    <!-- http://purl.obolibrary.org/obo/GAZ_00021999 -->

    <owl:NamedIndividual rdf:about="http://purl.obolibrary.org/obo/GAZ_00021999">
        <obo:RO_0001025 rdf:resource="http://purl.obolibrary.org/obo/GAZ_02000778"/>
        <oboInOwl:hasOBONamespace>GAZ</oboInOwl:hasOBONamespace>
        <oboInOwl:id>GAZ:00021999</oboInOwl:id>
        <rdfs:label>Tup District</rdfs:label>
    </owl:NamedIndividual>
    


    <!-- http://purl.obolibrary.org/obo/GAZ_00022000 -->

    <owl:NamedIndividual rdf:about="http://purl.obolibrary.org/obo/GAZ_00022000">
        <obo:RO_0001025 rdf:resource="http://purl.obolibrary.org/obo/GAZ_02000778"/>
        <oboInOwl:hasOBONamespace>GAZ</oboInOwl:hasOBONamespace>
        <oboInOwl:id>GAZ:00022000</oboInOwl:id>
        <rdfs:label>Ton District</rdfs:label>
    </owl:NamedIndividual>
    


    <!-- http://purl.obolibrary.org/obo/GAZ_00022001 -->

    <owl:NamedIndividual rdf:about="http://purl.obolibrary.org/obo/GAZ_00022001">
        <obo:RO_0001025 rdf:resource="http://purl.obolibrary.org/obo/GAZ_02000778"/>
        <oboInOwl:hasOBONamespace>GAZ</oboInOwl:hasOBONamespace>
        <oboInOwl:id>GAZ:00022001</oboInOwl:id>
        <rdfs:label>Issyk Kul District</rdfs:label>
    </owl:NamedIndividual>
    


    <!-- http://purl.obolibrary.org/obo/GAZ_00022002 -->

    <owl:NamedIndividual rdf:about="http://purl.obolibrary.org/obo/GAZ_00022002">
        <obo:RO_0001025 rdf:resource="http://purl.obolibrary.org/obo/GAZ_02000771"/>
        <oboInOwl:hasOBONamespace>GAZ</oboInOwl:hasOBONamespace>
        <oboInOwl:id>GAZ:00022002</oboInOwl:id>
        <rdfs:label>Chatkal District</rdfs:label>
    </owl:NamedIndividual>
    


    <!-- http://purl.obolibrary.org/obo/GAZ_00022003 -->

    <owl:NamedIndividual rdf:about="http://purl.obolibrary.org/obo/GAZ_00022003">
        <obo:RO_0001025 rdf:resource="http://purl.obolibrary.org/obo/GAZ_02000775"/>
        <oboInOwl:hasOBONamespace>GAZ</oboInOwl:hasOBONamespace>
        <oboInOwl:id>GAZ:00022003</oboInOwl:id>
        <rdfs:label>Jumgal District</rdfs:label>
    </owl:NamedIndividual>
    


    <!-- http://purl.obolibrary.org/obo/GAZ_00022004 -->

    <owl:NamedIndividual rdf:about="http://purl.obolibrary.org/obo/GAZ_00022004">
        <obo:RO_0001025 rdf:resource="http://purl.obolibrary.org/obo/GAZ_02000771"/>
        <oboInOwl:hasOBONamespace>GAZ</oboInOwl:hasOBONamespace>
        <oboInOwl:id>GAZ:00022004</oboInOwl:id>
        <rdfs:label>Suzak District</rdfs:label>
    </owl:NamedIndividual>
    


    <!-- http://purl.obolibrary.org/obo/GAZ_00022005 -->

    <owl:NamedIndividual rdf:about="http://purl.obolibrary.org/obo/GAZ_00022005">
        <obo:RO_0001025 rdf:resource="http://purl.obolibrary.org/obo/GAZ_02000771"/>
        <oboInOwl:hasOBONamespace>GAZ</oboInOwl:hasOBONamespace>
        <oboInOwl:id>GAZ:00022005</oboInOwl:id>
        <rdfs:label>Aksyi District</rdfs:label>
    </owl:NamedIndividual>
    


    <!-- http://purl.obolibrary.org/obo/GAZ_00022006 -->

    <owl:NamedIndividual rdf:about="http://purl.obolibrary.org/obo/GAZ_00022006">
        <obo:RO_0001025 rdf:resource="http://purl.obolibrary.org/obo/GAZ_02000771"/>
        <oboInOwl:hasOBONamespace>GAZ</oboInOwl:hasOBONamespace>
        <oboInOwl:id>GAZ:00022006</oboInOwl:id>
        <rdfs:label>Ala-Buka District</rdfs:label>
    </owl:NamedIndividual>
    


    <!-- http://purl.obolibrary.org/obo/GAZ_00022007 -->

    <owl:NamedIndividual rdf:about="http://purl.obolibrary.org/obo/GAZ_00022007">
        <obo:RO_0001025 rdf:resource="http://purl.obolibrary.org/obo/GAZ_02000771"/>
        <oboInOwl:hasOBONamespace>GAZ</oboInOwl:hasOBONamespace>
        <oboInOwl:id>GAZ:00022007</oboInOwl:id>
        <rdfs:label>Toktogul District</rdfs:label>
    </owl:NamedIndividual>
    


    <!-- http://purl.obolibrary.org/obo/GAZ_00022008 -->

    <owl:NamedIndividual rdf:about="http://purl.obolibrary.org/obo/GAZ_00022008">
        <obo:RO_0001025 rdf:resource="http://purl.obolibrary.org/obo/GAZ_02000771"/>
        <oboInOwl:hasOBONamespace>GAZ</oboInOwl:hasOBONamespace>
        <oboInOwl:id>GAZ:00022008</oboInOwl:id>
        <rdfs:label>Togus-Toro District</rdfs:label>
    </owl:NamedIndividual>
    


    <!-- http://purl.obolibrary.org/obo/GAZ_00022009 -->

    <owl:NamedIndividual rdf:about="http://purl.obolibrary.org/obo/GAZ_00022009">
        <obo:RO_0001025 rdf:resource="http://purl.obolibrary.org/obo/GAZ_02000775"/>
        <oboInOwl:hasOBONamespace>GAZ</oboInOwl:hasOBONamespace>
        <oboInOwl:id>GAZ:00022009</oboInOwl:id>
        <rdfs:label>Kochkor District</rdfs:label>
    </owl:NamedIndividual>
    


    <!-- http://purl.obolibrary.org/obo/GAZ_00022010 -->

    <owl:NamedIndividual rdf:about="http://purl.obolibrary.org/obo/GAZ_00022010">
        <obo:RO_0001025 rdf:resource="http://purl.obolibrary.org/obo/GAZ_02000771"/>
        <oboInOwl:hasOBONamespace>GAZ</oboInOwl:hasOBONamespace>
        <oboInOwl:id>GAZ:00022010</oboInOwl:id>
        <rdfs:label>Bazar-Korgon District</rdfs:label>
    </owl:NamedIndividual>
    


    <!-- http://purl.obolibrary.org/obo/GAZ_00022011 -->

    <owl:NamedIndividual rdf:about="http://purl.obolibrary.org/obo/GAZ_00022011">
        <obo:RO_0001025 rdf:resource="http://purl.obolibrary.org/obo/GAZ_02000775"/>
        <oboInOwl:hasOBONamespace>GAZ</oboInOwl:hasOBONamespace>
        <oboInOwl:id>GAZ:00022011</oboInOwl:id>
        <rdfs:label>Ak-Talaa District</rdfs:label>
    </owl:NamedIndividual>
    


    <!-- http://purl.obolibrary.org/obo/GAZ_00022012 -->

    <owl:NamedIndividual rdf:about="http://purl.obolibrary.org/obo/GAZ_00022012">
        <obo:RO_0001025 rdf:resource="http://purl.obolibrary.org/obo/GAZ_02000773"/>
        <oboInOwl:hasOBONamespace>GAZ</oboInOwl:hasOBONamespace>
        <oboInOwl:id>GAZ:00022012</oboInOwl:id>
        <rdfs:label>Kara-Buura District</rdfs:label>
    </owl:NamedIndividual>
    


    <!-- http://purl.obolibrary.org/obo/GAZ_00022013 -->

    <owl:NamedIndividual rdf:about="http://purl.obolibrary.org/obo/GAZ_00022013">
        <obo:RO_0001025 rdf:resource="http://purl.obolibrary.org/obo/GAZ_02000773"/>
        <oboInOwl:hasOBONamespace>GAZ</oboInOwl:hasOBONamespace>
        <oboInOwl:id>GAZ:00022013</oboInOwl:id>
        <rdfs:label>Bakai-Ata District</rdfs:label>
    </owl:NamedIndividual>
    


    <!-- http://purl.obolibrary.org/obo/GAZ_00022014 -->

    <owl:NamedIndividual rdf:about="http://purl.obolibrary.org/obo/GAZ_00022014">
        <obo:RO_0001025 rdf:resource="http://purl.obolibrary.org/obo/GAZ_02000773"/>
        <oboInOwl:hasOBONamespace>GAZ</oboInOwl:hasOBONamespace>
        <oboInOwl:id>GAZ:00022014</oboInOwl:id>
        <rdfs:label>Talas District</rdfs:label>
    </owl:NamedIndividual>
    


    <!-- http://purl.obolibrary.org/obo/GAZ_00022015 -->

    <owl:NamedIndividual rdf:about="http://purl.obolibrary.org/obo/GAZ_00022015">
        <obo:RO_0001025 rdf:resource="http://purl.obolibrary.org/obo/GAZ_02000773"/>
        <oboInOwl:hasOBONamespace>GAZ</oboInOwl:hasOBONamespace>
        <oboInOwl:id>GAZ:00022015</oboInOwl:id>
        <rdfs:label>Manas District</rdfs:label>
    </owl:NamedIndividual>
    


    <!-- http://purl.obolibrary.org/obo/GAZ_00022016 -->

    <owl:NamedIndividual rdf:about="http://purl.obolibrary.org/obo/GAZ_00022016">
        <obo:RO_0001025 rdf:resource="http://purl.obolibrary.org/obo/GAZ_02000776"/>
        <oboInOwl:hasOBONamespace>GAZ</oboInOwl:hasOBONamespace>
        <oboInOwl:id>GAZ:00022016</oboInOwl:id>
        <rdfs:label>Aravan District</rdfs:label>
    </owl:NamedIndividual>
    


    <!-- http://purl.obolibrary.org/obo/GAZ_00022017 -->

    <owl:NamedIndividual rdf:about="http://purl.obolibrary.org/obo/GAZ_00022017">
        <obo:RO_0001025 rdf:resource="http://purl.obolibrary.org/obo/GAZ_02000776"/>
        <oboInOwl:hasOBONamespace>GAZ</oboInOwl:hasOBONamespace>
        <oboInOwl:id>GAZ:00022017</oboInOwl:id>
        <rdfs:label>Kara-Kuldja District</rdfs:label>
    </owl:NamedIndividual>
    


    <!-- http://purl.obolibrary.org/obo/GAZ_00022018 -->

    <owl:NamedIndividual rdf:about="http://purl.obolibrary.org/obo/GAZ_00022018">
        <obo:RO_0001025 rdf:resource="http://purl.obolibrary.org/obo/GAZ_02000776"/>
        <oboInOwl:hasOBONamespace>GAZ</oboInOwl:hasOBONamespace>
        <oboInOwl:id>GAZ:00022018</oboInOwl:id>
        <rdfs:label>Ozgon District</rdfs:label>
    </owl:NamedIndividual>
    


    <!-- http://purl.obolibrary.org/obo/GAZ_00022019 -->

    <owl:NamedIndividual rdf:about="http://purl.obolibrary.org/obo/GAZ_00022019">
        <obo:RO_0001025 rdf:resource="http://purl.obolibrary.org/obo/GAZ_02000776"/>
        <oboInOwl:hasOBONamespace>GAZ</oboInOwl:hasOBONamespace>
        <oboInOwl:id>GAZ:00022019</oboInOwl:id>
        <rdfs:label>Alai District</rdfs:label>
    </owl:NamedIndividual>
    


    <!-- http://purl.obolibrary.org/obo/GAZ_00022020 -->

    <owl:NamedIndividual rdf:about="http://purl.obolibrary.org/obo/GAZ_00022020">
        <obo:RO_0001025 rdf:resource="http://purl.obolibrary.org/obo/GAZ_02000776"/>
        <oboInOwl:hasOBONamespace>GAZ</oboInOwl:hasOBONamespace>
        <oboInOwl:id>GAZ:00022020</oboInOwl:id>
        <rdfs:label>Chong-Alay District</rdfs:label>
    </owl:NamedIndividual>
    


    <!-- http://purl.obolibrary.org/obo/GAZ_00022021 -->

    <owl:NamedIndividual rdf:about="http://purl.obolibrary.org/obo/GAZ_00022021">
        <obo:RO_0001025 rdf:resource="http://purl.obolibrary.org/obo/GAZ_02000776"/>
        <oboInOwl:hasOBONamespace>GAZ</oboInOwl:hasOBONamespace>
        <oboInOwl:id>GAZ:00022021</oboInOwl:id>
        <rdfs:label>Nookat District</rdfs:label>
    </owl:NamedIndividual>
    


    <!-- http://purl.obolibrary.org/obo/GAZ_00022022 -->

    <owl:NamedIndividual rdf:about="http://purl.obolibrary.org/obo/GAZ_00022022">
        <obo:RO_0001025 rdf:resource="http://purl.obolibrary.org/obo/GAZ_02000776"/>
        <oboInOwl:hasOBONamespace>GAZ</oboInOwl:hasOBONamespace>
        <oboInOwl:id>GAZ:00022022</oboInOwl:id>
        <rdfs:label>Kara-Suu District</rdfs:label>
    </owl:NamedIndividual>
    


    <!-- http://purl.obolibrary.org/obo/GAZ_00051184 -->

    <owl:NamedIndividual rdf:about="http://purl.obolibrary.org/obo/GAZ_00051184">
        <obo:RO_0001025 rdf:resource="http://purl.obolibrary.org/obo/GAZ_02000778"/>
        <obo:IAO_0000115>An endorheic lake in the northern Tian Shan mountains in eastern Kyrgyzstan.</obo:IAO_0000115>
        <oboInOwl:hasOBONamespace>GAZ</oboInOwl:hasOBONamespace>
        <oboInOwl:id>GAZ:00051184</oboInOwl:id>
        <rdfs:label>Issyk Kul</rdfs:label>
    </owl:NamedIndividual>
    


    <!-- http://purl.obolibrary.org/obo/GAZ_00051185 -->

    <owl:NamedIndividual rdf:about="http://purl.obolibrary.org/obo/GAZ_00051185">
        <obo:RO_0001025 rdf:resource="http://purl.obolibrary.org/obo/GAZ_00006893"/>
        <obo:IAO_0000115>An endorheic alpine lake in the Tian Shan mountains in southern Kyrgyzstan.</obo:IAO_0000115>
        <oboInOwl:hasOBONamespace>GAZ</oboInOwl:hasOBONamespace>
        <oboInOwl:id>GAZ:00051185</oboInOwl:id>
        <rdfs:label>Chatyr-Kul</rdfs:label>
    </owl:NamedIndividual>
    


    <!-- http://purl.obolibrary.org/obo/GAZ_00051186 -->

    <owl:NamedIndividual rdf:about="http://purl.obolibrary.org/obo/GAZ_00051186">
        <obo:RO_0001025 rdf:resource="http://purl.obolibrary.org/obo/GAZ_00006893"/>
        <obo:RO_0001025 rdf:resource="http://purl.obolibrary.org/obo/GAZ_00008311"/>
        <obo:IAO_0000115>An endorheic alpine lake in the Tian Shan mountains in central Kyrgyzstan.</obo:IAO_0000115>
        <oboInOwl:hasOBONamespace>GAZ</oboInOwl:hasOBONamespace>
        <oboInOwl:id>GAZ:00051186</oboInOwl:id>
        <rdfs:label>Son-Kul</rdfs:label>
    </owl:NamedIndividual>
    


    <!-- http://purl.obolibrary.org/obo/GAZ_00052086 -->

    <owl:NamedIndividual rdf:about="http://purl.obolibrary.org/obo/GAZ_00052086">
        <obo:RO_0001025 rdf:resource="http://purl.obolibrary.org/obo/GAZ_02000776"/>
        <obo:IAO_0000115>An antimony/mercury deposit.</obo:IAO_0000115>
        <oboInOwl:hasOBONamespace>GAZ</oboInOwl:hasOBONamespace>
        <oboInOwl:id>GAZ:00052086</oboInOwl:id>
        <rdfs:label>Khaidarkan Sb-Hg deposit</rdfs:label>
    </owl:NamedIndividual>
    


    <!-- http://purl.obolibrary.org/obo/GAZ_00054856 -->

    <owl:NamedIndividual rdf:about="http://purl.obolibrary.org/obo/GAZ_00054856">
        <obo:RO_0001025 rdf:resource="http://purl.obolibrary.org/obo/GAZ_00008311"/>
        <obo:IAO_0000115>A fault-bounded trough located around and south of the city-oasis of Turfan, in the Xinjiang Autonomous Region in far western China, about 150 km southeast of the provincial capital Urumqi. It includes the second lowest exposed point on the Earth&apos;s surface, after the Dead Sea. It is located in the eastern part of the Tian Shan. It covers an area of 50,000 km2. The surrounding mountain ranges are: the central Tian Shan in the west, the Bogda Shan in the north-west, the Haerlike Shan in the north-west, and the Jueluotage Shan in the south. Beyond the surrounding mountain ranges lie the Junggar Basin in the north and the Tarim Basin in the south.</obo:IAO_0000115>
        <oboInOwl:hasOBONamespace>GAZ</oboInOwl:hasOBONamespace>
        <oboInOwl:id>GAZ:00054856</oboInOwl:id>
        <rdfs:label>Turfan Depression</rdfs:label>
    </owl:NamedIndividual>
    


    <!-- http://purl.obolibrary.org/obo/GAZ_00054858 -->

    <owl:NamedIndividual rdf:about="http://purl.obolibrary.org/obo/GAZ_00054858">
        <obo:RO_0001025 rdf:resource="http://purl.obolibrary.org/obo/GAZ_00008311"/>
        <obo:IAO_0000115>A volcano group in the Tianshan Mountains of Xinjiang Province in NW China contains the historically active cone of Pechan.</obo:IAO_0000115>
        <oboInOwl:hasOBONamespace>GAZ</oboInOwl:hasOBONamespace>
        <oboInOwl:id>GAZ:00054858</oboInOwl:id>
        <rdfs:label>Tianshan Volcanic Group</rdfs:label>
    </owl:NamedIndividual>
    


    <!-- http://purl.obolibrary.org/obo/GAZ_00054859 -->

    <owl:NamedIndividual rdf:about="http://purl.obolibrary.org/obo/GAZ_00054859">
        <obo:RO_0001025 rdf:resource="http://purl.obolibrary.org/obo/GAZ_00054858"/>
        <obo:IAO_0000115>A volcanic cone.</obo:IAO_0000115>
        <oboInOwl:hasOBONamespace>GAZ</oboInOwl:hasOBONamespace>
        <oboInOwl:id>GAZ:00054859</oboInOwl:id>
        <rdfs:label>Pechan Volcano</rdfs:label>
    </owl:NamedIndividual>
    


    <!-- http://purl.obolibrary.org/obo/GAZ_00057397 -->

    <owl:NamedIndividual rdf:about="http://purl.obolibrary.org/obo/GAZ_00057397">
        <obo:RO_0001025 rdf:resource="http://purl.obolibrary.org/obo/GAZ_00008311"/>
        <obo:IAO_0000115>A part of the Northern Tian Shan mountain system (ancient Mount Imeon) in Central Asia. It is the northernmost mountain range of Tian Shan stretching for about 350 km with maximal elevation of 4,973m (Talgar Peak).</obo:IAO_0000115>
        <oboInOwl:hasOBONamespace>GAZ</oboInOwl:hasOBONamespace>
        <oboInOwl:id>GAZ:00057397</oboInOwl:id>
        <rdfs:label>Trans-Ili Alatau</rdfs:label>
    </owl:NamedIndividual>
    


    <!-- http://purl.obolibrary.org/obo/GAZ_00057452 -->

    <owl:NamedIndividual rdf:about="http://purl.obolibrary.org/obo/GAZ_00057452">
        <obo:RO_0001025 rdf:resource="http://purl.obolibrary.org/obo/GAZ_00006893"/>
        <obo:RO_0001025 rdf:resource="http://purl.obolibrary.org/obo/GAZ_00008311"/>
        <obo:IAO_0000115>A mountain range that extends from the Tien Shan mountain range in Kyrgyzstan west into Tajikistan. The range runs approximately east and west. The southern slopes of the range drain into the Vakhsh River, a tributary of the Amu Darya. The streams that drain the northern slopes of the range are tributaries of the Syr Darya, and empty into the Ferghana Valley to the north of the range.</obo:IAO_0000115>
        <oboInOwl:hasOBONamespace>GAZ</oboInOwl:hasOBONamespace>
        <oboInOwl:id>GAZ:00057452</oboInOwl:id>
        <rdfs:label>Alay Mountains</rdfs:label>
    </owl:NamedIndividual>
    


    <!-- http://purl.obolibrary.org/obo/GAZ_00057491 -->

    <owl:NamedIndividual rdf:about="http://purl.obolibrary.org/obo/GAZ_00057491">
        <obo:RO_0001025 rdf:resource="http://purl.obolibrary.org/obo/GAZ_00006893"/>
        <obo:IAO_0000115>A mountain range of the Pamir Mountains (ancient Mount Imeon) between Kyrgyzstan and Tajikistan. Its northern end is the Alay Valley, and 150 miles to the south, it terminates into the valleys of Muksu and Markansu. The highest peak in the range is Lenin Peak.</obo:IAO_0000115>
        <oboInOwl:hasOBONamespace>GAZ</oboInOwl:hasOBONamespace>
        <oboInOwl:id>GAZ:00057491</oboInOwl:id>
        <rdfs:label>Trans-Alay Range</rdfs:label>
    </owl:NamedIndividual>
    


    <!-- http://purl.obolibrary.org/obo/GAZ_00058233 -->

    <owl:NamedIndividual rdf:about="http://purl.obolibrary.org/obo/GAZ_00058233">
        <obo:RO_0001025 rdf:resource="http://purl.obolibrary.org/obo/GAZ_00008311"/>
        <obo:IAO_0000115>A lake that lies on the north side of Bogda Peak of Tianshan Mountains, about 40 km east of Fukang County and 110 km east of Urumqi, in China. A World Heritage Site.</obo:IAO_0000115>
        <oboInOwl:hasOBONamespace>GAZ</oboInOwl:hasOBONamespace>
        <oboInOwl:id>GAZ:00058233</oboInOwl:id>
        <rdfs:label>Tianchi Lake</rdfs:label>
    </owl:NamedIndividual>
    


    <!-- http://purl.obolibrary.org/obo/GAZ_00058388 -->

    <owl:NamedIndividual rdf:about="http://purl.obolibrary.org/obo/GAZ_00058388">
        <obo:RO_0001025 rdf:resource="http://purl.obolibrary.org/obo/GAZ_02000771"/>
        <obo:IAO_0000115>A mountain lake and nature reserve in Jalal-Abad Province in Western Kyrgyzstan.</obo:IAO_0000115>
        <oboInOwl:hasOBONamespace>GAZ</oboInOwl:hasOBONamespace>
        <oboInOwl:id>GAZ:00058388</oboInOwl:id>
        <rdfs:label>Lake Sary-Chelek</rdfs:label>
    </owl:NamedIndividual>
    


    <!-- http://purl.obolibrary.org/obo/GAZ_00058389 -->

    <owl:NamedIndividual rdf:about="http://purl.obolibrary.org/obo/GAZ_00058389">
        <obo:RO_0001025 rdf:resource="http://purl.obolibrary.org/obo/GAZ_00058390"/>
        <obo:RO_0001025 rdf:resource="http://purl.obolibrary.org/obo/GAZ_02000771"/>
        <obo:IAO_0000115>A reservoir located in the Jalal-Abad Province of Kyrgyzstan, is the largest of the reservoirs on the Naryn River.</obo:IAO_0000115>
        <oboInOwl:hasOBONamespace>GAZ</oboInOwl:hasOBONamespace>
        <oboInOwl:id>GAZ:00058389</oboInOwl:id>
        <rdfs:label>Toktogul Reservoir</rdfs:label>
    </owl:NamedIndividual>
    


    <!-- http://purl.obolibrary.org/obo/GAZ_00058390 -->

    <owl:NamedIndividual rdf:about="http://purl.obolibrary.org/obo/GAZ_00058390">
        <obo:RO_0001025 rdf:resource="http://purl.obolibrary.org/obo/GAZ_00006893"/>
        <obo:IAO_0000115>A river that rises in the Tien Shan mountains in Kyrgyzstan, Central Asia, flowing west through the Fergana Valley into Uzbekistan. Here it confluences with the Kara Darya River to form the Syr Darya.</obo:IAO_0000115>
        <oboInOwl:hasOBONamespace>GAZ</oboInOwl:hasOBONamespace>
        <oboInOwl:id>GAZ:00058390</oboInOwl:id>
        <rdfs:label>Naryn River</rdfs:label>
    </owl:NamedIndividual>
    


    <!-- http://purl.obolibrary.org/obo/GAZ_00058500 -->

    <owl:NamedIndividual rdf:about="http://purl.obolibrary.org/obo/GAZ_00058500">
        <obo:RO_0001025 rdf:resource="http://purl.obolibrary.org/obo/GAZ_00008373"/>
        <obo:IAO_0000115>A Central Asian river, and one of the main rivers of the nation of Tajikistan. It is a tributary of the Amu Darya river. The river&apos;s source lies in Kyrgyzstan; it then flows through Tajikistan for a length of 524 km before joining the Panj River to form the Amu Darya at the border of Tajikistan and Afghanistan.</obo:IAO_0000115>
        <oboInOwl:hasOBONamespace>GAZ</oboInOwl:hasOBONamespace>
        <oboInOwl:id>GAZ:00058500</oboInOwl:id>
        <rdfs:label>Vakhsh River</rdfs:label>
    </owl:NamedIndividual>
    


    <!-- http://purl.obolibrary.org/obo/GAZ_00058501 -->

    <owl:NamedIndividual rdf:about="http://purl.obolibrary.org/obo/GAZ_00058501">
        <obo:RO_0001025 rdf:resource="http://purl.obolibrary.org/obo/GAZ_00058500"/>
        <obo:IAO_0000115>A reservoir formed bu the Nurek Dam on the Vakhsh River in Tajikistan.</obo:IAO_0000115>
        <oboInOwl:hasOBONamespace>GAZ</oboInOwl:hasOBONamespace>
        <oboInOwl:id>GAZ:00058501</oboInOwl:id>
        <rdfs:label>Nurek</rdfs:label>
    </owl:NamedIndividual>
    


    <!-- http://purl.obolibrary.org/obo/GAZ_00089988 -->

    <owl:NamedIndividual rdf:about="http://purl.obolibrary.org/obo/GAZ_00089988">
        <obo:RO_0001025 rdf:resource="http://purl.obolibrary.org/obo/GAZ_00006893"/>
        <obo:IAO_0000115>An alpine national park in Kyrgyzstan, established in 1976 and located approximately 40 km south of the capital city of Bishkek.</obo:IAO_0000115>
        <oboInOwl:hasOBONamespace>GAZ</oboInOwl:hasOBONamespace>
        <oboInOwl:id>GAZ:00089988</oboInOwl:id>
        <rdfs:label>Ala Archa National Park</rdfs:label>
    </owl:NamedIndividual>
    


    <!-- http://purl.obolibrary.org/obo/GAZ_00103909 -->

    <owl:NamedIndividual rdf:about="http://purl.obolibrary.org/obo/GAZ_00103909">
        <obo:RO_0001025 rdf:resource="http://purl.obolibrary.org/obo/GAZ_00006893"/>
        <obo:IAO_0000115>A mountain range. The Alaiskiy Range is located in the South of Kyrgyzstan, separates the Fergana Valley from Alaiskiy Valley. On West the range joins the Turkestanskiy Range and is as if its extension to the East for 400 km to the Chinese border.</obo:IAO_0000115>
        <oboInOwl:hasOBONamespace>GAZ</oboInOwl:hasOBONamespace>
        <oboInOwl:id>GAZ:00103909</oboInOwl:id>
        <rdfs:label>Alaiskiy Khrebet</rdfs:label>
    </owl:NamedIndividual>
    


    <!-- http://purl.obolibrary.org/obo/GAZ_00114469 -->

    <owl:NamedIndividual rdf:about="http://purl.obolibrary.org/obo/GAZ_00114469">
        <obo:RO_0001025 rdf:resource="http://purl.obolibrary.org/obo/GAZ_00008311"/>
        <obo:IAO_0000115>A mountain range that is part of the eastern Tien Shan mountains, and located in Xinjiang, not far from Urumqi. The highest elevation is Bogda Feng, at 5445 m.</obo:IAO_0000115>
        <oboInOwl:hasOBONamespace>GAZ</oboInOwl:hasOBONamespace>
        <oboInOwl:id>GAZ:00114469</oboInOwl:id>
        <rdfs:label>Bogda Shan</rdfs:label>
    </owl:NamedIndividual>
    


    <!-- http://purl.obolibrary.org/obo/GAZ_00117272 -->

    <owl:NamedIndividual rdf:about="http://purl.obolibrary.org/obo/GAZ_00117272">
        <obo:RO_0001025 rdf:resource="http://purl.obolibrary.org/obo/GAZ_00054856"/>
        <obo:IAO_0000115>A saline lake in a closed basin in the Turfan region of inland Xinjiang. The basin has very steep slopes and is surrounded by high mountains. The Ayding basin originated as a fault depression. The lake water is supplied by runoff from eight rivers and by some groundwater inflow. The water in the lake is extremely saline, with a salt content of &gt; 200 g/l. The lake had an area of 22.5 km2 in 1958 and a mean water depth of 0.8m, but had been reduced to 5 km2 and a mean water depth below 0.5 m by 1996.</obo:IAO_0000115>
        <oboInOwl:hasOBONamespace>GAZ</oboInOwl:hasOBONamespace>
        <oboInOwl:id>GAZ:00117272</oboInOwl:id>
        <rdfs:label>Aiding Hu</rdfs:label>
    </owl:NamedIndividual>
    


    <!-- http://purl.obolibrary.org/obo/GAZ_00129974 -->

    <owl:NamedIndividual rdf:about="http://purl.obolibrary.org/obo/GAZ_00129974">
        <obo:RO_0001025 rdf:resource="http://purl.obolibrary.org/obo/GAZ_00008311"/>
        <obo:IAO_0000115>A protected area located in the east part of the Tianshan Mountains on the southern brim of the Kurbantungut desert of the Zhunger Basin.</obo:IAO_0000115>
        <oboInOwl:hasOBONamespace>GAZ</oboInOwl:hasOBONamespace>
        <oboInOwl:id>GAZ:00129974</oboInOwl:id>
        <rdfs:label>Bogeda Nature Reserve</rdfs:label>
    </owl:NamedIndividual>
    


    <!-- http://purl.obolibrary.org/obo/GAZ_00247302 -->

    <owl:NamedIndividual rdf:about="http://purl.obolibrary.org/obo/GAZ_00247302">
        <obo:RO_0001025 rdf:resource="http://purl.obolibrary.org/obo/GAZ_00008311"/>
        <obo:IAO_0000115>A protected area. Includes a vast complex of small freshwater lakes, ponds and marshes in an intermontane basin in the Tian Shan mountains. The marshes are fed by numerous rivers and streams from the surrounding hills, and drain east through a gorge into Bosten Hu and Bo Hu Marshes Located in Hejing County, 200 km northwest of Kuerle. Established 1980.</obo:IAO_0000115>
        <oboInOwl:hasOBONamespace>GAZ</oboInOwl:hasOBONamespace>
        <oboInOwl:id>GAZ:00247302</oboInOwl:id>
        <rdfs:label>Bayinbuluke Nature Reserve</rdfs:label>
    </owl:NamedIndividual>
    


    <!-- http://purl.obolibrary.org/obo/GAZ_00250942 -->

    <owl:NamedIndividual rdf:about="http://purl.obolibrary.org/obo/GAZ_00250942">
        <rdf:type rdf:resource="http://purl.obolibrary.org/obo/ENVO_00000020"/>
        <obo:RO_0001025 rdf:resource="http://purl.obolibrary.org/obo/GAZ_02000776"/>
        <obo:IAO_0000115>A broad, dry valley running east-west across most of southern Osh Province, Kyrgyzstan.</obo:IAO_0000115>
        <oboInOwl:hasOBONamespace>GAZ</oboInOwl:hasOBONamespace>
        <oboInOwl:id>GAZ:00250942</oboInOwl:id>
        <rdfs:label>Alay Valley</rdfs:label>
    </owl:NamedIndividual>
    


    <!-- http://purl.obolibrary.org/obo/GAZ_00250943 -->

    <owl:NamedIndividual rdf:about="http://purl.obolibrary.org/obo/GAZ_00250943">
        <obo:RO_0001025 rdf:resource="http://purl.obolibrary.org/obo/GAZ_00058500"/>
        <obo:IAO_0000115>A dam. Constructed 1961-1980.</obo:IAO_0000115>
        <oboInOwl:hasOBONamespace>GAZ</oboInOwl:hasOBONamespace>
        <oboInOwl:id>GAZ:00250943</oboInOwl:id>
        <rdfs:label>Nurek Dam</rdfs:label>
    </owl:NamedIndividual>
    


    <!-- http://purl.obolibrary.org/obo/GAZ_00360612 -->

    <owl:NamedIndividual rdf:about="http://purl.obolibrary.org/obo/GAZ_00360612">
        <obo:IAO_0000115>A former republic of the Soviet Union.</obo:IAO_0000115>
        <oboInOwl:hasOBONamespace>GAZ</oboInOwl:hasOBONamespace>
        <oboInOwl:id>GAZ:00360612</oboInOwl:id>
        <rdfs:label>[Former] Moldavian Soviet Socialist Republic</rdfs:label>
    </owl:NamedIndividual>
    


    <!-- http://purl.obolibrary.org/obo/GAZ_00405959 -->

    <owl:NamedIndividual rdf:about="http://purl.obolibrary.org/obo/GAZ_00405959">
        <obo:IAO_0000115>A short-lived republic of the Soviet Union. It consisted of Georgia, Armenia, and Azerbaijan, traditionally known as the Transcaucasian Republics, being separated from Russia by the Caucasus Mountains. 1922-1936.</obo:IAO_0000115>
        <oboInOwl:hasOBONamespace>GAZ</oboInOwl:hasOBONamespace>
        <oboInOwl:id>GAZ:00405959</oboInOwl:id>
        <rdfs:label>[Former] Transcaucasian Socialist Federative Soviet Republic</rdfs:label>
    </owl:NamedIndividual>
    


    <!-- http://purl.obolibrary.org/obo/GAZ_00405960 -->

    <owl:NamedIndividual rdf:about="http://purl.obolibrary.org/obo/GAZ_00405960">
        <obo:IAO_0000115>A former republic of the USSR.</obo:IAO_0000115>
        <oboInOwl:hasOBONamespace>GAZ</oboInOwl:hasOBONamespace>
        <oboInOwl:id>GAZ:00405960</oboInOwl:id>
        <rdfs:label>[Former] Georgian Soviet Socialist Republic</rdfs:label>
    </owl:NamedIndividual>
    


    <!-- http://purl.obolibrary.org/obo/GAZ_00405961 -->

    <owl:NamedIndividual rdf:about="http://purl.obolibrary.org/obo/GAZ_00405961">
        <obo:IAO_0000115>A former republic of the USSR. 1922-1991.</obo:IAO_0000115>
        <oboInOwl:hasOBONamespace>GAZ</oboInOwl:hasOBONamespace>
        <oboInOwl:id>GAZ:00405961</oboInOwl:id>
        <rdfs:label>[Former] Armenian Soviet Socialist Republic</rdfs:label>
    </owl:NamedIndividual>
    


    <!-- http://purl.obolibrary.org/obo/GAZ_00405962 -->

    <owl:NamedIndividual rdf:about="http://purl.obolibrary.org/obo/GAZ_00405962">
        <obo:IAO_0000115>A former republic of the USSR. 1937-1990.</obo:IAO_0000115>
        <oboInOwl:hasOBONamespace>GAZ</oboInOwl:hasOBONamespace>
        <oboInOwl:id>GAZ:00405962</oboInOwl:id>
        <rdfs:label>[Former] Azerbaijan Soviet Socialist Republic</rdfs:label>
    </owl:NamedIndividual>
    


    <!-- http://purl.obolibrary.org/obo/GAZ_00405963 -->

    <owl:NamedIndividual rdf:about="http://purl.obolibrary.org/obo/GAZ_00405963">
        <oboInOwl:hasOBONamespace>GAZ</oboInOwl:hasOBONamespace>
        <oboInOwl:id>GAZ:00405963</oboInOwl:id>
        <rdfs:label>[Former] Russian Soviet Federative Socialist Republic</rdfs:label>
    </owl:NamedIndividual>
    


    <!-- http://purl.obolibrary.org/obo/GAZ_00405964 -->

    <owl:NamedIndividual rdf:about="http://purl.obolibrary.org/obo/GAZ_00405964">
        <oboInOwl:hasOBONamespace>GAZ</oboInOwl:hasOBONamespace>
        <oboInOwl:id>GAZ:00405964</oboInOwl:id>
        <rdfs:label>[Former[ Ukrainian Soviet Socialist Republic</rdfs:label>
    </owl:NamedIndividual>
    


    <!-- http://purl.obolibrary.org/obo/GAZ_00405965 -->

    <owl:NamedIndividual rdf:about="http://purl.obolibrary.org/obo/GAZ_00405965">
        <oboInOwl:hasOBONamespace>GAZ</oboInOwl:hasOBONamespace>
        <oboInOwl:id>GAZ:00405965</oboInOwl:id>
        <rdfs:label>[Former] Byelorussian Soviet Socialist Republic</rdfs:label>
    </owl:NamedIndividual>
    


    <!-- http://purl.obolibrary.org/obo/GAZ_00405966 -->

    <owl:NamedIndividual rdf:about="http://purl.obolibrary.org/obo/GAZ_00405966">
        <oboInOwl:hasOBONamespace>GAZ</oboInOwl:hasOBONamespace>
        <oboInOwl:id>GAZ:00405966</oboInOwl:id>
        <rdfs:label>[Former] Uzbek Soviet Socialist Republic</rdfs:label>
    </owl:NamedIndividual>
    


    <!-- http://purl.obolibrary.org/obo/GAZ_00405967 -->

    <owl:NamedIndividual rdf:about="http://purl.obolibrary.org/obo/GAZ_00405967">
        <oboInOwl:hasOBONamespace>GAZ</oboInOwl:hasOBONamespace>
        <oboInOwl:id>GAZ:00405967</oboInOwl:id>
        <rdfs:label>[Former] Kazakh Soviet Socialist Republic</rdfs:label>
    </owl:NamedIndividual>
    


    <!-- http://purl.obolibrary.org/obo/GAZ_00405968 -->

    <owl:NamedIndividual rdf:about="http://purl.obolibrary.org/obo/GAZ_00405968">
        <oboInOwl:hasOBONamespace>GAZ</oboInOwl:hasOBONamespace>
        <oboInOwl:id>GAZ:00405968</oboInOwl:id>
        <rdfs:label>[Former] Lithuanian Soviet Socialist Republic</rdfs:label>
    </owl:NamedIndividual>
    


    <!-- http://purl.obolibrary.org/obo/GAZ_00405969 -->

    <owl:NamedIndividual rdf:about="http://purl.obolibrary.org/obo/GAZ_00405969">
        <oboInOwl:hasOBONamespace>GAZ</oboInOwl:hasOBONamespace>
        <oboInOwl:id>GAZ:00405969</oboInOwl:id>
        <rdfs:label>[Former] Kirghiz Soviet Socialist Republic</rdfs:label>
    </owl:NamedIndividual>
    


    <!-- http://purl.obolibrary.org/obo/GAZ_00405970 -->

    <owl:NamedIndividual rdf:about="http://purl.obolibrary.org/obo/GAZ_00405970">
        <oboInOwl:hasOBONamespace>GAZ</oboInOwl:hasOBONamespace>
        <oboInOwl:id>GAZ:00405970</oboInOwl:id>
        <rdfs:label>[Former] Latvian Soviet Socialist Republic</rdfs:label>
    </owl:NamedIndividual>
    


    <!-- http://purl.obolibrary.org/obo/GAZ_00405971 -->

    <owl:NamedIndividual rdf:about="http://purl.obolibrary.org/obo/GAZ_00405971">
        <oboInOwl:hasOBONamespace>GAZ</oboInOwl:hasOBONamespace>
        <oboInOwl:id>GAZ:00405971</oboInOwl:id>
        <rdfs:label>[Former] Turkmen Soviet Socialist Republic</rdfs:label>
    </owl:NamedIndividual>
    


    <!-- http://purl.obolibrary.org/obo/GAZ_00405972 -->

    <owl:NamedIndividual rdf:about="http://purl.obolibrary.org/obo/GAZ_00405972">
        <oboInOwl:hasOBONamespace>GAZ</oboInOwl:hasOBONamespace>
        <oboInOwl:id>GAZ:00405972</oboInOwl:id>
        <rdfs:label>[Former] Estonian Soviet Socialist Republic</rdfs:label>
    </owl:NamedIndividual>
    


    <!-- http://purl.obolibrary.org/obo/GAZ_00405973 -->

    <owl:NamedIndividual rdf:about="http://purl.obolibrary.org/obo/GAZ_00405973">
        <oboInOwl:hasOBONamespace>GAZ</oboInOwl:hasOBONamespace>
        <oboInOwl:id>GAZ:00405973</oboInOwl:id>
        <rdfs:label>[Former] Tajik Soviet Socialist Republic</rdfs:label>
    </owl:NamedIndividual>
    


    <!-- http://purl.obolibrary.org/obo/GAZ_00415845 -->

    <owl:NamedIndividual rdf:about="http://purl.obolibrary.org/obo/GAZ_00415845">
        <obo:RO_0001025 rdf:resource="http://purl.obolibrary.org/obo/GAZ_00022022"/>
        <obo:IAO_0000115>A populated place. An eclave in Uzbek territory.</obo:IAO_0000115>
        <oboInOwl:hasOBONamespace>GAZ</oboInOwl:hasOBONamespace>
        <oboInOwl:id>GAZ:00415845</oboInOwl:id>
        <rdfs:label>Barak ail</rdfs:label>
    </owl:NamedIndividual>
    


    <!-- http://purl.obolibrary.org/obo/GAZ_00415848 -->

    <owl:NamedIndividual rdf:about="http://purl.obolibrary.org/obo/GAZ_00415848">
        <obo:IAO_0000115>A jamoat in northern Tajikistan. It is located in Isfara District in Sughd province. Vorukh forms part of an exclave of Tajikistan within Kyrgyzstan</obo:IAO_0000115>
        <oboInOwl:hasOBONamespace>GAZ</oboInOwl:hasOBONamespace>
        <oboInOwl:id>GAZ:00415848</oboInOwl:id>
        <rdfs:label>Vorukh</rdfs:label>
    </owl:NamedIndividual>
    


    <!-- http://purl.obolibrary.org/obo/GAZ_02000771 -->

    <owl:NamedIndividual rdf:about="http://purl.obolibrary.org/obo/GAZ_02000771"/>
    


    <!-- http://purl.obolibrary.org/obo/GAZ_02000772 -->

    <owl:NamedIndividual rdf:about="http://purl.obolibrary.org/obo/GAZ_02000772"/>
    


    <!-- http://purl.obolibrary.org/obo/GAZ_02000773 -->

    <owl:NamedIndividual rdf:about="http://purl.obolibrary.org/obo/GAZ_02000773"/>
    


    <!-- http://purl.obolibrary.org/obo/GAZ_02000774 -->

    <owl:NamedIndividual rdf:about="http://purl.obolibrary.org/obo/GAZ_02000774"/>
    


    <!-- http://purl.obolibrary.org/obo/GAZ_02000775 -->

    <owl:NamedIndividual rdf:about="http://purl.obolibrary.org/obo/GAZ_02000775"/>
    


    <!-- http://purl.obolibrary.org/obo/GAZ_02000776 -->

    <owl:NamedIndividual rdf:about="http://purl.obolibrary.org/obo/GAZ_02000776"/>
    


    <!-- http://purl.obolibrary.org/obo/GAZ_02000777 -->

    <owl:NamedIndividual rdf:about="http://purl.obolibrary.org/obo/GAZ_02000777"/>
    


    <!-- http://purl.obolibrary.org/obo/GAZ_02000778 -->

    <owl:NamedIndividual rdf:about="http://purl.obolibrary.org/obo/GAZ_02000778"/>
    


    <!-- http://purl.obolibrary.org/obo/GAZ_02000779 -->

    <owl:NamedIndividual rdf:about="http://purl.obolibrary.org/obo/GAZ_02000779">
        <obo:RO_0001025 rdf:resource="http://purl.obolibrary.org/obo/GAZ_00006893"/>
    </owl:NamedIndividual>
    


    <!-- 
    ///////////////////////////////////////////////////////////////////////////////////////
    //
    // Annotations
    //
    ///////////////////////////////////////////////////////////////////////////////////////
     -->

    <rdf:Description rdf:about="http://purl.obolibrary.org/obo/GAZ_00009463">
        <rdfs:label>Oblast (Kyrgyzstan)</rdfs:label>
        <oboInOwl:hasOBONamespace>GAZ</oboInOwl:hasOBONamespace>
        <oboInOwl:id>GAZ:00009463</oboInOwl:id>
    </rdf:Description>
    <rdf:Description rdf:about="http://purl.obolibrary.org/obo/GAZ_02000771">
        <oboInOwl:id>GAZ:02000771</oboInOwl:id>
        <oboInOwl:hasOBONamespace>GAZ</oboInOwl:hasOBONamespace>
        <rdfs:label>Jalal-Abad Oblast</rdfs:label>
    </rdf:Description>
    <rdf:Description rdf:about="http://purl.obolibrary.org/obo/GAZ_02000772">
        <oboInOwl:id>GAZ:02000772</oboInOwl:id>
        <rdfs:label>Chuy Oblast</rdfs:label>
        <oboInOwl:hasOBONamespace>GAZ</oboInOwl:hasOBONamespace>
    </rdf:Description>
    <rdf:Description rdf:about="http://purl.obolibrary.org/obo/GAZ_02000773">
        <oboInOwl:id>GAZ:02000773</oboInOwl:id>
        <oboInOwl:hasOBONamespace>GAZ</oboInOwl:hasOBONamespace>
        <rdfs:label>Talas Oblast</rdfs:label>
    </rdf:Description>
    <rdf:Description rdf:about="http://purl.obolibrary.org/obo/GAZ_02000774">
        <oboInOwl:hasOBONamespace>GAZ</oboInOwl:hasOBONamespace>
        <oboInOwl:id>GAZ:02000774</oboInOwl:id>
        <rdfs:label>Bishkek City</rdfs:label>
    </rdf:Description>
    <rdf:Description rdf:about="http://purl.obolibrary.org/obo/GAZ_02000775">
        <oboInOwl:id>GAZ:02000775</oboInOwl:id>
        <oboInOwl:hasOBONamespace>GAZ</oboInOwl:hasOBONamespace>
        <rdfs:label>Naryn Oblast</rdfs:label>
    </rdf:Description>
    <rdf:Description rdf:about="http://purl.obolibrary.org/obo/GAZ_02000776">
        <oboInOwl:id>GAZ:02000776</oboInOwl:id>
        <oboInOwl:hasOBONamespace>GAZ</oboInOwl:hasOBONamespace>
        <rdfs:label>Osh Oblast</rdfs:label>
    </rdf:Description>
    <rdf:Description rdf:about="http://purl.obolibrary.org/obo/GAZ_02000777">
        <oboInOwl:id>GAZ:02000777</oboInOwl:id>
        <rdfs:label>Batken Oblast</rdfs:label>
        <oboInOwl:hasOBONamespace>GAZ</oboInOwl:hasOBONamespace>
    </rdf:Description>
    <rdf:Description rdf:about="http://purl.obolibrary.org/obo/GAZ_02000778">
        <oboInOwl:id>GAZ:02000778</oboInOwl:id>
        <rdfs:label>Ysyk-Kol Oblast</rdfs:label>
        <oboInOwl:hasOBONamespace>GAZ</oboInOwl:hasOBONamespace>
    </rdf:Description>
    <rdf:Description rdf:about="http://purl.obolibrary.org/obo/GAZ_02000779">
        <oboInOwl:hasOBONamespace>GAZ</oboInOwl:hasOBONamespace>
        <rdfs:label>City (Kyrgyzstan)</rdfs:label>
        <oboInOwl:id>GAZ:02000779</oboInOwl:id>
    </rdf:Description>
</rdf:RDF>



<!-- Generated by the OWL API (version 4.5.6) https://github.com/owlcs/owlapi -->

