<?xml version="1.0"?>
<rdf:RDF xmlns="http://purl.obolibrary.org/obo/gaz/subsets/countries/Liechtenstein.owl#"
     xml:base="http://purl.obolibrary.org/obo/gaz/subsets/countries/Liechtenstein.owl"
     xmlns:obo="http://purl.obolibrary.org/obo/"
     xmlns:owl="http://www.w3.org/2002/07/owl#"
     xmlns:rdf="http://www.w3.org/1999/02/22-rdf-syntax-ns#"
     xmlns:xml="http://www.w3.org/XML/1998/namespace"
     xmlns:xsd="http://www.w3.org/2001/XMLSchema#"
     xmlns:rdfs="http://www.w3.org/2000/01/rdf-schema#"
     xmlns:oboInOwl="http://www.geneontology.org/formats/oboInOwl#">
    <owl:Ontology rdf:about="http://purl.obolibrary.org/obo/gaz/subsets/countries/Liechtenstein.owl">
        <owl:imports rdf:resource="http://purl.obolibrary.org/obo/gaz/imports/envo_import.owl"/>
        <owl:imports rdf:resource="http://purl.obolibrary.org/obo/gaz/imports/ro_import.owl"/>
    </owl:Ontology>
    


    <!-- 
    ///////////////////////////////////////////////////////////////////////////////////////
    //
    // Annotation properties
    //
    ///////////////////////////////////////////////////////////////////////////////////////
     -->

    


    <!-- http://purl.obolibrary.org/obo/IAO_0000115 -->

    <owl:AnnotationProperty rdf:about="http://purl.obolibrary.org/obo/IAO_0000115"/>
    


    <!-- http://www.geneontology.org/formats/oboInOwl#hasOBONamespace -->

    <owl:AnnotationProperty rdf:about="http://www.geneontology.org/formats/oboInOwl#hasOBONamespace"/>
    


    <!-- http://www.geneontology.org/formats/oboInOwl#id -->

    <owl:AnnotationProperty rdf:about="http://www.geneontology.org/formats/oboInOwl#id"/>
    


    <!-- 
    ///////////////////////////////////////////////////////////////////////////////////////
    //
    // Object Properties
    //
    ///////////////////////////////////////////////////////////////////////////////////////
     -->

    


    <!-- http://purl.obolibrary.org/obo/RO_0001025 -->

    <owl:ObjectProperty rdf:about="http://purl.obolibrary.org/obo/RO_0001025"/>
    


    <!-- 
    ///////////////////////////////////////////////////////////////////////////////////////
    //
    // Classes
    //
    ///////////////////////////////////////////////////////////////////////////////////////
     -->

    


    <!-- http://purl.obolibrary.org/obo/ENVO_00000029 -->

    <owl:Class rdf:about="http://purl.obolibrary.org/obo/ENVO_00000029"/>
    


    <!-- http://purl.obolibrary.org/obo/ENVO_00000080 -->

    <owl:Class rdf:about="http://purl.obolibrary.org/obo/ENVO_00000080"/>
    


    <!-- http://purl.obolibrary.org/obo/ENVO_00000100 -->

    <owl:Class rdf:about="http://purl.obolibrary.org/obo/ENVO_00000100"/>
    


    <!-- http://purl.obolibrary.org/obo/ENVO_00000106 -->

    <owl:Class rdf:about="http://purl.obolibrary.org/obo/ENVO_00000106"/>
    


    <!-- http://purl.obolibrary.org/obo/ENVO_00000423 -->

    <owl:Class rdf:about="http://purl.obolibrary.org/obo/ENVO_00000423"/>
    


    <!-- http://purl.obolibrary.org/obo/ENVO_00000856 -->

    <owl:Class rdf:about="http://purl.obolibrary.org/obo/ENVO_00000856"/>
    


    <!-- http://purl.obolibrary.org/obo/GAZ_00005367 -->

    <owl:Class rdf:about="http://purl.obolibrary.org/obo/GAZ_00005367"/>
    


    <!-- http://purl.obolibrary.org/obo/GAZ_00005544 -->

    <owl:Class rdf:about="http://purl.obolibrary.org/obo/GAZ_00005544"/>
    


    <!-- http://purl.obolibrary.org/obo/GAZ_00007412 -->

    <owl:Class rdf:about="http://purl.obolibrary.org/obo/GAZ_00007412"/>
    


    <!-- http://purl.obolibrary.org/obo/GAZ_00008262 -->

    <owl:Class rdf:about="http://purl.obolibrary.org/obo/GAZ_00008262"/>
    


    <!-- http://purl.obolibrary.org/obo/GAZ_00009543 -->

    <owl:Class rdf:about="http://purl.obolibrary.org/obo/GAZ_00009543"/>
    


    <!-- http://purl.obolibrary.org/obo/GAZ_00013805 -->

    <owl:Class rdf:about="http://purl.obolibrary.org/obo/GAZ_00013805">
        <rdfs:subClassOf rdf:resource="http://purl.obolibrary.org/obo/GAZ_00009543"/>
    </owl:Class>
    


    <!-- http://purl.obolibrary.org/obo/GAZ_00013806 -->

    <owl:Class rdf:about="http://purl.obolibrary.org/obo/GAZ_00013806">
        <rdfs:subClassOf rdf:resource="http://purl.obolibrary.org/obo/GAZ_00009543"/>
        <obo:IAO_0000115>A municipality.</obo:IAO_0000115>
        <oboInOwl:hasOBONamespace>GAZ</oboInOwl:hasOBONamespace>
        <oboInOwl:id>GAZ:00013806</oboInOwl:id>
        <rdfs:label>Commune of Schaan</rdfs:label>
    </owl:Class>
    


    <!-- http://purl.obolibrary.org/obo/GAZ_00013807 -->

    <owl:Class rdf:about="http://purl.obolibrary.org/obo/GAZ_00013807">
        <rdfs:subClassOf rdf:resource="http://purl.obolibrary.org/obo/GAZ_00009543"/>
    </owl:Class>
    


    <!-- http://purl.obolibrary.org/obo/GAZ_00013808 -->

    <owl:Class rdf:about="http://purl.obolibrary.org/obo/GAZ_00013808">
        <rdfs:subClassOf rdf:resource="http://purl.obolibrary.org/obo/GAZ_00009543"/>
    </owl:Class>
    


    <!-- http://purl.obolibrary.org/obo/GAZ_00013809 -->

    <owl:Class rdf:about="http://purl.obolibrary.org/obo/GAZ_00013809">
        <rdfs:subClassOf rdf:resource="http://purl.obolibrary.org/obo/GAZ_00009543"/>
    </owl:Class>
    


    <!-- http://purl.obolibrary.org/obo/GAZ_00013810 -->

    <owl:Class rdf:about="http://purl.obolibrary.org/obo/GAZ_00013810">
        <rdfs:subClassOf rdf:resource="http://purl.obolibrary.org/obo/GAZ_00009543"/>
    </owl:Class>
    


    <!-- http://purl.obolibrary.org/obo/GAZ_00013811 -->

    <owl:Class rdf:about="http://purl.obolibrary.org/obo/GAZ_00013811">
        <rdfs:subClassOf rdf:resource="http://purl.obolibrary.org/obo/GAZ_00009543"/>
    </owl:Class>
    


    <!-- http://purl.obolibrary.org/obo/GAZ_00013812 -->

    <owl:Class rdf:about="http://purl.obolibrary.org/obo/GAZ_00013812">
        <rdfs:subClassOf rdf:resource="http://purl.obolibrary.org/obo/GAZ_00009543"/>
    </owl:Class>
    


    <!-- http://purl.obolibrary.org/obo/GAZ_00013813 -->

    <owl:Class rdf:about="http://purl.obolibrary.org/obo/GAZ_00013813">
        <rdfs:subClassOf rdf:resource="http://purl.obolibrary.org/obo/GAZ_00009543"/>
    </owl:Class>
    


    <!-- http://purl.obolibrary.org/obo/GAZ_00013814 -->

    <owl:Class rdf:about="http://purl.obolibrary.org/obo/GAZ_00013814">
        <rdfs:subClassOf rdf:resource="http://purl.obolibrary.org/obo/GAZ_00009543"/>
    </owl:Class>
    


    <!-- http://purl.obolibrary.org/obo/GAZ_00013815 -->

    <owl:Class rdf:about="http://purl.obolibrary.org/obo/GAZ_00013815">
        <rdfs:subClassOf rdf:resource="http://purl.obolibrary.org/obo/GAZ_00009543"/>
    </owl:Class>
    


    <!-- http://purl.obolibrary.org/obo/GAZ_00013816 -->

    <owl:Class rdf:about="http://purl.obolibrary.org/obo/GAZ_00013816">
        <rdfs:subClassOf rdf:resource="http://purl.obolibrary.org/obo/GAZ_00013817"/>
    </owl:Class>
    


    <!-- http://purl.obolibrary.org/obo/GAZ_00013817 -->

    <owl:Class rdf:about="http://purl.obolibrary.org/obo/GAZ_00013817"/>
    


    <!-- http://purl.obolibrary.org/obo/GAZ_00060215 -->

    <owl:Class rdf:about="http://purl.obolibrary.org/obo/GAZ_00060215">
        <rdfs:subClassOf rdf:resource="http://purl.obolibrary.org/obo/GAZ_00060232"/>
        <obo:IAO_0000115>A lake in the Queyras Valley.</obo:IAO_0000115>
        <oboInOwl:hasOBONamespace>GAZ</oboInOwl:hasOBONamespace>
        <oboInOwl:id>GAZ:00060215</oboInOwl:id>
        <rdfs:label>Lac Egorgeou</rdfs:label>
    </owl:Class>
    


    <!-- http://purl.obolibrary.org/obo/GAZ_00060232 -->

    <owl:Class rdf:about="http://purl.obolibrary.org/obo/GAZ_00060232"/>
    


    <!-- http://purl.obolibrary.org/obo/GAZ_00060233 -->

    <owl:Class rdf:about="http://purl.obolibrary.org/obo/GAZ_00060233"/>
    


    <!-- http://purl.obolibrary.org/obo/GAZ_00060235 -->

    <owl:Class rdf:about="http://purl.obolibrary.org/obo/GAZ_00060235">
        <rdfs:subClassOf rdf:resource="http://purl.obolibrary.org/obo/GAZ_00060233"/>
        <obo:IAO_0000115>A lake in the Queyras Valley.</obo:IAO_0000115>
        <oboInOwl:hasOBONamespace>GAZ</oboInOwl:hasOBONamespace>
        <oboInOwl:id>GAZ:00060235</oboInOwl:id>
        <rdfs:label>Lac de la Roue</rdfs:label>
    </owl:Class>
    


    <!-- http://purl.obolibrary.org/obo/GAZ_00060236 -->

    <owl:Class rdf:about="http://purl.obolibrary.org/obo/GAZ_00060236">
        <rdfs:subClassOf rdf:resource="http://purl.obolibrary.org/obo/GAZ_00060233"/>
        <obo:IAO_0000115>A lake in the Queyras Valley.</obo:IAO_0000115>
        <oboInOwl:hasOBONamespace>GAZ</oboInOwl:hasOBONamespace>
        <oboInOwl:id>GAZ:00060236</oboInOwl:id>
        <rdfs:label>Lac Soulier</rdfs:label>
    </owl:Class>
    


    <!-- http://purl.obolibrary.org/obo/GAZ_00060238 -->

    <owl:Class rdf:about="http://purl.obolibrary.org/obo/GAZ_00060238">
        <rdfs:subClassOf rdf:resource="http://purl.obolibrary.org/obo/GAZ_00060232"/>
        <obo:IAO_0000115>A lake in the Queyras Valley.</obo:IAO_0000115>
        <oboInOwl:hasOBONamespace>GAZ</oboInOwl:hasOBONamespace>
        <oboInOwl:id>GAZ:00060238</oboInOwl:id>
        <rdfs:label>Lac Baricle</rdfs:label>
    </owl:Class>
    


    <!-- http://purl.obolibrary.org/obo/GAZ_00060239 -->

    <owl:Class rdf:about="http://purl.obolibrary.org/obo/GAZ_00060239">
        <rdfs:subClassOf rdf:resource="http://purl.obolibrary.org/obo/GAZ_00060232"/>
        <obo:IAO_0000115>A lake in the Queyras Valley.</obo:IAO_0000115>
        <oboInOwl:hasOBONamespace>GAZ</oboInOwl:hasOBONamespace>
        <oboInOwl:id>GAZ:00060239</oboInOwl:id>
        <rdfs:label>Lac Foreant</rdfs:label>
    </owl:Class>
    


    <!-- http://purl.obolibrary.org/obo/GAZ_00060240 -->

    <owl:Class rdf:about="http://purl.obolibrary.org/obo/GAZ_00060240"/>
    


    <!-- http://purl.obolibrary.org/obo/GAZ_00060246 -->

    <owl:Class rdf:about="http://purl.obolibrary.org/obo/GAZ_00060246">
        <rdfs:subClassOf rdf:resource="http://purl.obolibrary.org/obo/GAZ_00060240"/>
        <obo:IAO_0000115>A lake in the Queyras Valley.</obo:IAO_0000115>
        <oboInOwl:hasOBONamespace>GAZ</oboInOwl:hasOBONamespace>
        <oboInOwl:id>GAZ:00060246</oboInOwl:id>
        <rdfs:label>Lac du Grand-Laus</rdfs:label>
    </owl:Class>
    


    <!-- http://purl.obolibrary.org/obo/GAZ_00060247 -->

    <owl:Class rdf:about="http://purl.obolibrary.org/obo/GAZ_00060247">
        <rdfs:subClassOf rdf:resource="http://purl.obolibrary.org/obo/GAZ_00060240"/>
        <obo:IAO_0000115>A lake in the Queyras Valley.</obo:IAO_0000115>
        <oboInOwl:hasOBONamespace>GAZ</oboInOwl:hasOBONamespace>
        <oboInOwl:id>GAZ:00060247</oboInOwl:id>
        <rdfs:label>Lac Mezan</rdfs:label>
    </owl:Class>
    


    <!-- http://purl.obolibrary.org/obo/GAZ_00060248 -->

    <owl:Class rdf:about="http://purl.obolibrary.org/obo/GAZ_00060248">
        <rdfs:subClassOf rdf:resource="http://purl.obolibrary.org/obo/GAZ_00060240"/>
        <obo:IAO_0000115>A lake in the Queyras Valley.</obo:IAO_0000115>
        <oboInOwl:hasOBONamespace>GAZ</oboInOwl:hasOBONamespace>
        <oboInOwl:id>GAZ:00060248</oboInOwl:id>
        <rdfs:label>Lac du Petit-Laus</rdfs:label>
    </owl:Class>
    


    <!-- http://purl.obolibrary.org/obo/GAZ_00060392 -->

    <owl:Class rdf:about="http://purl.obolibrary.org/obo/GAZ_00060392">
        <rdfs:subClassOf rdf:resource="http://purl.obolibrary.org/obo/GAZ_00060404"/>
        <obo:IAO_0000115>A lake in La chaine de Belledonne.</obo:IAO_0000115>
        <oboInOwl:hasOBONamespace>GAZ</oboInOwl:hasOBONamespace>
        <oboInOwl:id>GAZ:00060392</oboInOwl:id>
        <rdfs:label>Lac Cottepens</rdfs:label>
    </owl:Class>
    


    <!-- http://purl.obolibrary.org/obo/GAZ_00060393 -->

    <owl:Class rdf:about="http://purl.obolibrary.org/obo/GAZ_00060393">
        <rdfs:subClassOf rdf:resource="http://purl.obolibrary.org/obo/GAZ_00060404"/>
        <obo:IAO_0000115>A lake in La chaine de Belledonne.</obo:IAO_0000115>
        <oboInOwl:hasOBONamespace>GAZ</oboInOwl:hasOBONamespace>
        <oboInOwl:id>GAZ:00060393</oboInOwl:id>
        <rdfs:label>Lac Carre</rdfs:label>
    </owl:Class>
    


    <!-- http://purl.obolibrary.org/obo/GAZ_00060397 -->

    <owl:Class rdf:about="http://purl.obolibrary.org/obo/GAZ_00060397">
        <rdfs:subClassOf rdf:resource="http://purl.obolibrary.org/obo/GAZ_00060404"/>
        <obo:IAO_0000115>A lake in La chaine de Belledonne at 2248m.</obo:IAO_0000115>
        <oboInOwl:hasOBONamespace>GAZ</oboInOwl:hasOBONamespace>
        <oboInOwl:id>GAZ:00060397</oboInOwl:id>
        <rdfs:label>Lac Blanc</rdfs:label>
    </owl:Class>
    


    <!-- http://purl.obolibrary.org/obo/GAZ_00060403 -->

    <owl:Class rdf:about="http://purl.obolibrary.org/obo/GAZ_00060403">
        <rdfs:subClassOf rdf:resource="http://purl.obolibrary.org/obo/GAZ_00060404"/>
        <obo:IAO_0000115>A lake in La chaine de Belledonne.</obo:IAO_0000115>
        <oboInOwl:hasOBONamespace>GAZ</oboInOwl:hasOBONamespace>
        <oboInOwl:id>GAZ:00060403</oboInOwl:id>
        <rdfs:label>Lac de la Motte</rdfs:label>
    </owl:Class>
    


    <!-- http://purl.obolibrary.org/obo/GAZ_00060404 -->

    <owl:Class rdf:about="http://purl.obolibrary.org/obo/GAZ_00060404"/>
    


    <!-- http://purl.obolibrary.org/obo/GAZ_00060405 -->

    <owl:Class rdf:about="http://purl.obolibrary.org/obo/GAZ_00060405">
        <rdfs:subClassOf rdf:resource="http://purl.obolibrary.org/obo/GAZ_00060404"/>
        <obo:IAO_0000115>A lake in La chaine de Belledonne at 2091m.</obo:IAO_0000115>
        <oboInOwl:hasOBONamespace>GAZ</oboInOwl:hasOBONamespace>
        <oboInOwl:id>GAZ:00060405</oboInOwl:id>
        <rdfs:label>Lac Noir</rdfs:label>
    </owl:Class>
    


    <!-- http://purl.obolibrary.org/obo/GAZ_00060406 -->

    <owl:Class rdf:about="http://purl.obolibrary.org/obo/GAZ_00060406">
        <rdfs:subClassOf rdf:resource="http://purl.obolibrary.org/obo/GAZ_00060404"/>
        <obo:IAO_0000115>A lake in La chaine de Belledonne.</obo:IAO_0000115>
        <oboInOwl:hasOBONamespace>GAZ</oboInOwl:hasOBONamespace>
        <oboInOwl:id>GAZ:00060406</oboInOwl:id>
        <rdfs:label>Lac de la Corne</rdfs:label>
    </owl:Class>
    


    <!-- http://purl.obolibrary.org/obo/GAZ_00060409 -->

    <owl:Class rdf:about="http://purl.obolibrary.org/obo/GAZ_00060409">
        <rdfs:subClassOf rdf:resource="http://purl.obolibrary.org/obo/GAZ_00060404"/>
        <obo:IAO_0000115>A lake in La chaine de Belledonne.</obo:IAO_0000115>
        <oboInOwl:hasOBONamespace>GAZ</oboInOwl:hasOBONamespace>
        <oboInOwl:id>GAZ:00060409</oboInOwl:id>
        <rdfs:label>Lac Jeplan</rdfs:label>
    </owl:Class>
    


    <!-- http://purl.obolibrary.org/obo/GAZ_00060410 -->

    <owl:Class rdf:about="http://purl.obolibrary.org/obo/GAZ_00060410">
        <rdfs:subClassOf rdf:resource="http://purl.obolibrary.org/obo/GAZ_00060404"/>
    </owl:Class>
    


    <!-- http://purl.obolibrary.org/obo/GAZ_00060412 -->

    <owl:Class rdf:about="http://purl.obolibrary.org/obo/GAZ_00060412">
        <rdfs:subClassOf rdf:resource="http://purl.obolibrary.org/obo/GAZ_00060404"/>
        <obo:IAO_0000115>A lake in La chaine de Belledonne.</obo:IAO_0000115>
        <oboInOwl:hasOBONamespace>GAZ</oboInOwl:hasOBONamespace>
        <oboInOwl:id>GAZ:00060412</oboInOwl:id>
        <rdfs:label>Lac de la Sagne</rdfs:label>
    </owl:Class>
    


    <!-- http://purl.obolibrary.org/obo/GAZ_00060415 -->

    <owl:Class rdf:about="http://purl.obolibrary.org/obo/GAZ_00060415">
        <rdfs:subClassOf rdf:resource="http://purl.obolibrary.org/obo/GAZ_00060404"/>
        <obo:IAO_0000115>A lake in La chaine de Belledonne.</obo:IAO_0000115>
        <oboInOwl:hasOBONamespace>GAZ</oboInOwl:hasOBONamespace>
        <oboInOwl:id>GAZ:00060415</oboInOwl:id>
        <rdfs:label>Lac de l&apos;Agnelin</rdfs:label>
    </owl:Class>
    


    <!-- http://purl.obolibrary.org/obo/GAZ_00144360 -->

    <owl:Class rdf:about="http://purl.obolibrary.org/obo/GAZ_00144360">
        <obo:IAO_0000115>A 350 km long river in northern France, western Belgium and the southwestern part of the Netherlands. The headwaters of the Scheldt are in Gouy, in the Aisne department of northern France. It flows north through Cambrai and Valenciennes, and enters Belgium near Tournai. In Ghent, where it receives the Lys, its main tributary, the Scheldt turns east. Near Antwerp, the largest city on its banks, the Scheldt flows west into the Netherlands towards the North Sea.</obo:IAO_0000115>
        <oboInOwl:hasOBONamespace>GAZ</oboInOwl:hasOBONamespace>
        <oboInOwl:id>GAZ:00144360</oboInOwl:id>
        <rdfs:label>Scheldt</rdfs:label>
    </owl:Class>
    


    <!-- http://purl.obolibrary.org/obo/GAZ_00597288 -->

    <owl:Class rdf:about="http://purl.obolibrary.org/obo/GAZ_00597288">
        <oboInOwl:hasOBONamespace>GAZ</oboInOwl:hasOBONamespace>
        <oboInOwl:id>GAZ:00597288</oboInOwl:id>
        <rdfs:label>Autenbrunnengraben [W of Bonlander Strasse]</rdfs:label>
    </owl:Class>
    


    <!-- http://purl.obolibrary.org/obo/GAZ_00597654 -->

    <owl:Class rdf:about="http://purl.obolibrary.org/obo/GAZ_00597654">
        <obo:IAO_0000115>A river in Germany near Freiburg.</obo:IAO_0000115>
        <oboInOwl:hasOBONamespace>GAZ</oboInOwl:hasOBONamespace>
        <oboInOwl:id>GAZ:00597654</oboInOwl:id>
        <rdfs:label>Dreisam</rdfs:label>
    </owl:Class>
    


    <!-- http://purl.obolibrary.org/obo/GAZ_00605262 -->

    <owl:Class rdf:about="http://purl.obolibrary.org/obo/GAZ_00605262">
        <obo:IAO_0000115>A river.</obo:IAO_0000115>
        <oboInOwl:hasOBONamespace>GAZ</oboInOwl:hasOBONamespace>
        <oboInOwl:id>GAZ:00605262</oboInOwl:id>
        <rdfs:label>Fallenbach</rdfs:label>
    </owl:Class>
    


    <!-- http://purl.obolibrary.org/obo/GAZ_00607653 -->

    <owl:Class rdf:about="http://purl.obolibrary.org/obo/GAZ_00607653">
        <obo:IAO_0000115>A river.</obo:IAO_0000115>
        <oboInOwl:hasOBONamespace>GAZ</oboInOwl:hasOBONamespace>
        <oboInOwl:id>GAZ:00607653</oboInOwl:id>
        <rdfs:label>Schwabinger Bach</rdfs:label>
    </owl:Class>
    


    <!-- http://purl.obolibrary.org/obo/GAZ_00607654 -->

    <owl:Class rdf:about="http://purl.obolibrary.org/obo/GAZ_00607654">
        <obo:IAO_0000115>A river.</obo:IAO_0000115>
        <oboInOwl:hasOBONamespace>GAZ</oboInOwl:hasOBONamespace>
        <oboInOwl:id>GAZ:00607654</oboInOwl:id>
        <rdfs:label>Eisbach</rdfs:label>
    </owl:Class>
    


    <!-- http://purl.obolibrary.org/obo/GAZ_00619830 -->

    <owl:Class rdf:about="http://purl.obolibrary.org/obo/GAZ_00619830"/>
    


    <!-- http://purl.obolibrary.org/obo/GAZ_00619831 -->

    <owl:Class rdf:about="http://purl.obolibrary.org/obo/GAZ_00619831">
        <obo:IAO_0000115>A river.</obo:IAO_0000115>
        <oboInOwl:hasOBONamespace>GAZ</oboInOwl:hasOBONamespace>
        <oboInOwl:id>GAZ:00619831</oboInOwl:id>
        <rdfs:label>Dreimuhlenbch</rdfs:label>
    </owl:Class>
    


    <!-- http://purl.obolibrary.org/obo/GAZ_00619832 -->

    <owl:Class rdf:about="http://purl.obolibrary.org/obo/GAZ_00619832">
        <obo:IAO_0000115>A river.</obo:IAO_0000115>
        <oboInOwl:hasOBONamespace>GAZ</oboInOwl:hasOBONamespace>
        <oboInOwl:id>GAZ:00619832</oboInOwl:id>
        <rdfs:label>Grosser Stadtbach</rdfs:label>
    </owl:Class>
    


    <!-- http://purl.obolibrary.org/obo/GAZ_00619833 -->

    <owl:Class rdf:about="http://purl.obolibrary.org/obo/GAZ_00619833">
        <obo:IAO_0000115>A river.</obo:IAO_0000115>
        <oboInOwl:hasOBONamespace>GAZ</oboInOwl:hasOBONamespace>
        <oboInOwl:id>GAZ:00619833</oboInOwl:id>
        <rdfs:label>Westmuhlbach</rdfs:label>
    </owl:Class>
    


    <!-- http://purl.obolibrary.org/obo/GAZ_00619834 -->

    <owl:Class rdf:about="http://purl.obolibrary.org/obo/GAZ_00619834">
        <obo:IAO_0000115>A river.</obo:IAO_0000115>
        <oboInOwl:hasOBONamespace>GAZ</oboInOwl:hasOBONamespace>
        <oboInOwl:id>GAZ:00619834</oboInOwl:id>
        <rdfs:label>Pesenbach</rdfs:label>
    </owl:Class>
    


    <!-- http://purl.obolibrary.org/obo/GAZ_00619835 -->

    <owl:Class rdf:about="http://purl.obolibrary.org/obo/GAZ_00619835">
        <obo:IAO_0000115>A river.</obo:IAO_0000115>
        <oboInOwl:hasOBONamespace>GAZ</oboInOwl:hasOBONamespace>
        <oboInOwl:id>GAZ:00619835</oboInOwl:id>
        <rdfs:label>Bleicherbachl</rdfs:label>
    </owl:Class>
    


    <!-- http://purl.obolibrary.org/obo/GAZ_00619836 -->

    <owl:Class rdf:about="http://purl.obolibrary.org/obo/GAZ_00619836">
        <obo:IAO_0000115>A river.</obo:IAO_0000115>
        <oboInOwl:hasOBONamespace>GAZ</oboInOwl:hasOBONamespace>
        <oboInOwl:id>GAZ:00619836</oboInOwl:id>
        <rdfs:label>Blererbachl</rdfs:label>
    </owl:Class>
    


    <!-- http://purl.obolibrary.org/obo/GAZ_00619837 -->

    <owl:Class rdf:about="http://purl.obolibrary.org/obo/GAZ_00619837">
        <obo:IAO_0000115>A river.</obo:IAO_0000115>
        <oboInOwl:hasOBONamespace>GAZ</oboInOwl:hasOBONamespace>
        <oboInOwl:id>GAZ:00619837</oboInOwl:id>
        <rdfs:label>Glockenbach</rdfs:label>
    </owl:Class>
    


    <!-- http://purl.obolibrary.org/obo/GAZ_00619838 -->

    <owl:Class rdf:about="http://purl.obolibrary.org/obo/GAZ_00619838">
        <obo:IAO_0000115>A river.</obo:IAO_0000115>
        <oboInOwl:hasOBONamespace>GAZ</oboInOwl:hasOBONamespace>
        <oboInOwl:id>GAZ:00619838</oboInOwl:id>
        <rdfs:label>Mahlmuhlbach</rdfs:label>
    </owl:Class>
    


    <!-- http://purl.obolibrary.org/obo/GAZ_00619839 -->

    <owl:Class rdf:about="http://purl.obolibrary.org/obo/GAZ_00619839">
        <obo:IAO_0000115>A river.</obo:IAO_0000115>
        <oboInOwl:hasOBONamespace>GAZ</oboInOwl:hasOBONamespace>
        <oboInOwl:id>GAZ:00619839</oboInOwl:id>
        <rdfs:label>Gipsmuhlkanak</rdfs:label>
    </owl:Class>
    


    <!-- http://purl.obolibrary.org/obo/GAZ_00619840 -->

    <owl:Class rdf:about="http://purl.obolibrary.org/obo/GAZ_00619840">
        <obo:IAO_0000115>A river.</obo:IAO_0000115>
        <oboInOwl:hasOBONamespace>GAZ</oboInOwl:hasOBONamespace>
        <oboInOwl:id>GAZ:00619840</oboInOwl:id>
        <rdfs:label>Grosser Angerbach</rdfs:label>
    </owl:Class>
    


    <!-- http://purl.obolibrary.org/obo/GAZ_00619841 -->

    <owl:Class rdf:about="http://purl.obolibrary.org/obo/GAZ_00619841">
        <obo:IAO_0000115>A river.</obo:IAO_0000115>
        <oboInOwl:hasOBONamespace>GAZ</oboInOwl:hasOBONamespace>
        <oboInOwl:id>GAZ:00619841</oboInOwl:id>
        <rdfs:label>Kleiner Angerbach</rdfs:label>
    </owl:Class>
    


    <!-- http://purl.obolibrary.org/obo/GAZ_00619842 -->

    <owl:Class rdf:about="http://purl.obolibrary.org/obo/GAZ_00619842">
        <obo:IAO_0000115>A river.</obo:IAO_0000115>
        <oboInOwl:hasOBONamespace>GAZ</oboInOwl:hasOBONamespace>
        <oboInOwl:id>GAZ:00619842</oboInOwl:id>
        <rdfs:label>Fabrikbach</rdfs:label>
    </owl:Class>
    


    <!-- http://purl.obolibrary.org/obo/GAZ_00619843 -->

    <owl:Class rdf:about="http://purl.obolibrary.org/obo/GAZ_00619843">
        <obo:IAO_0000115>A river.</obo:IAO_0000115>
        <oboInOwl:hasOBONamespace>GAZ</oboInOwl:hasOBONamespace>
        <oboInOwl:id>GAZ:00619843</oboInOwl:id>
        <rdfs:label>Apothekerbachl</rdfs:label>
    </owl:Class>
    


    <!-- http://purl.obolibrary.org/obo/GAZ_00619844 -->

    <owl:Class rdf:about="http://purl.obolibrary.org/obo/GAZ_00619844">
        <obo:IAO_0000115>A river.</obo:IAO_0000115>
        <oboInOwl:hasOBONamespace>GAZ</oboInOwl:hasOBONamespace>
        <oboInOwl:id>GAZ:00619844</oboInOwl:id>
        <rdfs:label>Einschuttbach</rdfs:label>
    </owl:Class>
    


    <!-- http://purl.obolibrary.org/obo/GAZ_00619845 -->

    <owl:Class rdf:about="http://purl.obolibrary.org/obo/GAZ_00619845">
        <obo:IAO_0000115>A river.</obo:IAO_0000115>
        <oboInOwl:hasOBONamespace>GAZ</oboInOwl:hasOBONamespace>
        <oboInOwl:id>GAZ:00619845</oboInOwl:id>
        <rdfs:label>Farbergrabenbach</rdfs:label>
    </owl:Class>
    


    <!-- http://purl.obolibrary.org/obo/GAZ_00619847 -->

    <owl:Class rdf:about="http://purl.obolibrary.org/obo/GAZ_00619847">
        <obo:IAO_0000115>A river.</obo:IAO_0000115>
        <oboInOwl:hasOBONamespace>GAZ</oboInOwl:hasOBONamespace>
        <oboInOwl:id>GAZ:00619847</oboInOwl:id>
        <rdfs:label>Holzartenkanal</rdfs:label>
    </owl:Class>
    


    <!-- http://purl.obolibrary.org/obo/GAZ_00619848 -->

    <owl:Class rdf:about="http://purl.obolibrary.org/obo/GAZ_00619848">
        <obo:IAO_0000115>A river.</obo:IAO_0000115>
        <oboInOwl:hasOBONamespace>GAZ</oboInOwl:hasOBONamespace>
        <oboInOwl:id>GAZ:00619848</oboInOwl:id>
        <rdfs:label>Eiener Kanal</rdfs:label>
    </owl:Class>
    


    <!-- http://purl.obolibrary.org/obo/GAZ_00619849 -->

    <owl:Class rdf:about="http://purl.obolibrary.org/obo/GAZ_00619849">
        <obo:IAO_0000115>A river.</obo:IAO_0000115>
        <oboInOwl:hasOBONamespace>GAZ</oboInOwl:hasOBONamespace>
        <oboInOwl:id>GAZ:00619849</oboInOwl:id>
        <rdfs:label>Brauhausbachl</rdfs:label>
    </owl:Class>
    


    <!-- http://purl.obolibrary.org/obo/GAZ_00619850 -->

    <owl:Class rdf:about="http://purl.obolibrary.org/obo/GAZ_00619850">
        <obo:IAO_0000115>A river.</obo:IAO_0000115>
        <oboInOwl:hasOBONamespace>GAZ</oboInOwl:hasOBONamespace>
        <oboInOwl:id>GAZ:00619850</oboInOwl:id>
        <rdfs:label>Ostlicher Stadtgrabenbach</rdfs:label>
    </owl:Class>
    


    <!-- http://purl.obolibrary.org/obo/GAZ_00619851 -->

    <owl:Class rdf:about="http://purl.obolibrary.org/obo/GAZ_00619851">
        <obo:IAO_0000115>A river.</obo:IAO_0000115>
        <oboInOwl:hasOBONamespace>GAZ</oboInOwl:hasOBONamespace>
        <oboInOwl:id>GAZ:00619851</oboInOwl:id>
        <rdfs:label>Westlicher Stadtgrabekbach</rdfs:label>
    </owl:Class>
    


    <!-- http://purl.obolibrary.org/obo/GAZ_00619852 -->

    <owl:Class rdf:about="http://purl.obolibrary.org/obo/GAZ_00619852">
        <obo:IAO_0000115>A river.</obo:IAO_0000115>
        <oboInOwl:hasOBONamespace>GAZ</oboInOwl:hasOBONamespace>
        <oboInOwl:id>GAZ:00619852</oboInOwl:id>
        <rdfs:label>Feuerbachl</rdfs:label>
    </owl:Class>
    


    <!-- http://purl.obolibrary.org/obo/GAZ_00619853 -->

    <owl:Class rdf:about="http://purl.obolibrary.org/obo/GAZ_00619853">
        <obo:IAO_0000115>A river.</obo:IAO_0000115>
        <oboInOwl:hasOBONamespace>GAZ</oboInOwl:hasOBONamespace>
        <oboInOwl:id>GAZ:00619853</oboInOwl:id>
        <rdfs:label>Feuerhausbachl</rdfs:label>
    </owl:Class>
    


    <!-- http://purl.obolibrary.org/obo/GAZ_00619854 -->

    <owl:Class rdf:about="http://purl.obolibrary.org/obo/GAZ_00619854">
        <obo:IAO_0000115>A river.</obo:IAO_0000115>
        <oboInOwl:hasOBONamespace>GAZ</oboInOwl:hasOBONamespace>
        <oboInOwl:id>GAZ:00619854</oboInOwl:id>
        <rdfs:label>Fischerbach</rdfs:label>
    </owl:Class>
    


    <!-- http://purl.obolibrary.org/obo/GAZ_00619856 -->

    <owl:Class rdf:about="http://purl.obolibrary.org/obo/GAZ_00619856">
        <obo:IAO_0000115>A river.</obo:IAO_0000115>
        <oboInOwl:hasOBONamespace>GAZ</oboInOwl:hasOBONamespace>
        <oboInOwl:id>GAZ:00619856</oboInOwl:id>
        <rdfs:label>Gernbach</rdfs:label>
    </owl:Class>
    


    <!-- http://purl.obolibrary.org/obo/GAZ_00619857 -->

    <owl:Class rdf:about="http://purl.obolibrary.org/obo/GAZ_00619857">
        <obo:IAO_0000115>A river.</obo:IAO_0000115>
        <oboInOwl:hasOBONamespace>GAZ</oboInOwl:hasOBONamespace>
        <oboInOwl:id>GAZ:00619857</oboInOwl:id>
        <rdfs:label>Gewurzmuhkanal</rdfs:label>
    </owl:Class>
    


    <!-- http://purl.obolibrary.org/obo/GAZ_00619858 -->

    <owl:Class rdf:about="http://purl.obolibrary.org/obo/GAZ_00619858">
        <obo:IAO_0000115>A river.</obo:IAO_0000115>
        <oboInOwl:hasOBONamespace>GAZ</oboInOwl:hasOBONamespace>
        <oboInOwl:id>GAZ:00619858</oboInOwl:id>
        <rdfs:label>Gewurzmuhlbach</rdfs:label>
    </owl:Class>
    


    <!-- http://purl.obolibrary.org/obo/GAZ_00619859 -->

    <owl:Class rdf:about="http://purl.obolibrary.org/obo/GAZ_00619859">
        <obo:IAO_0000115>A river.</obo:IAO_0000115>
        <oboInOwl:hasOBONamespace>GAZ</oboInOwl:hasOBONamespace>
        <oboInOwl:id>GAZ:00619859</oboInOwl:id>
        <rdfs:label>Hacklmuhlbach</rdfs:label>
    </owl:Class>
    


    <!-- http://purl.obolibrary.org/obo/GAZ_00619860 -->

    <owl:Class rdf:about="http://purl.obolibrary.org/obo/GAZ_00619860">
        <obo:IAO_0000115>A river.</obo:IAO_0000115>
        <oboInOwl:hasOBONamespace>GAZ</oboInOwl:hasOBONamespace>
        <oboInOwl:id>GAZ:00619860</oboInOwl:id>
        <rdfs:label>Heiliggeistmuhlbach</rdfs:label>
    </owl:Class>
    


    <!-- http://purl.obolibrary.org/obo/GAZ_00619861 -->

    <owl:Class rdf:about="http://purl.obolibrary.org/obo/GAZ_00619861">
        <obo:IAO_0000115>A river.</obo:IAO_0000115>
        <oboInOwl:hasOBONamespace>GAZ</oboInOwl:hasOBONamespace>
        <oboInOwl:id>GAZ:00619861</oboInOwl:id>
        <rdfs:label>Hochbruckbach</rdfs:label>
    </owl:Class>
    


    <!-- http://purl.obolibrary.org/obo/GAZ_00619862 -->

    <owl:Class rdf:about="http://purl.obolibrary.org/obo/GAZ_00619862">
        <obo:IAO_0000115>A river.</obo:IAO_0000115>
        <oboInOwl:hasOBONamespace>GAZ</oboInOwl:hasOBONamespace>
        <oboInOwl:id>GAZ:00619862</oboInOwl:id>
        <rdfs:label>Hofgrabenbach</rdfs:label>
    </owl:Class>
    


    <!-- http://purl.obolibrary.org/obo/GAZ_00619863 -->

    <owl:Class rdf:about="http://purl.obolibrary.org/obo/GAZ_00619863">
        <obo:IAO_0000115>A river.</obo:IAO_0000115>
        <oboInOwl:hasOBONamespace>GAZ</oboInOwl:hasOBONamespace>
        <oboInOwl:id>GAZ:00619863</oboInOwl:id>
        <rdfs:label>Hofbrunnwerkkanal</rdfs:label>
    </owl:Class>
    


    <!-- http://purl.obolibrary.org/obo/GAZ_00619864 -->

    <owl:Class rdf:about="http://purl.obolibrary.org/obo/GAZ_00619864">
        <obo:IAO_0000115>A river.</obo:IAO_0000115>
        <oboInOwl:hasOBONamespace>GAZ</oboInOwl:hasOBONamespace>
        <oboInOwl:id>GAZ:00619864</oboInOwl:id>
        <rdfs:label>Koglmuhlbach</rdfs:label>
    </owl:Class>
    


    <!-- http://purl.obolibrary.org/obo/GAZ_00619865 -->

    <owl:Class rdf:about="http://purl.obolibrary.org/obo/GAZ_00619865">
        <obo:IAO_0000115>A river.</obo:IAO_0000115>
        <oboInOwl:hasOBONamespace>GAZ</oboInOwl:hasOBONamespace>
        <oboInOwl:id>GAZ:00619865</oboInOwl:id>
        <rdfs:label>Hofhammerschmiedbach</rdfs:label>
    </owl:Class>
    


    <!-- http://purl.obolibrary.org/obo/GAZ_00619866 -->

    <owl:Class rdf:about="http://purl.obolibrary.org/obo/GAZ_00619866">
        <obo:IAO_0000115>A river.</obo:IAO_0000115>
        <oboInOwl:hasOBONamespace>GAZ</oboInOwl:hasOBONamespace>
        <oboInOwl:id>GAZ:00619866</oboInOwl:id>
        <rdfs:label>Hofsagmuhlbach</rdfs:label>
    </owl:Class>
    


    <!-- http://purl.obolibrary.org/obo/GAZ_00619867 -->

    <owl:Class rdf:about="http://purl.obolibrary.org/obo/GAZ_00619867">
        <obo:IAO_0000115>A river.</obo:IAO_0000115>
        <oboInOwl:hasOBONamespace>GAZ</oboInOwl:hasOBONamespace>
        <oboInOwl:id>GAZ:00619867</oboInOwl:id>
        <rdfs:label>Holzgartenkanal</rdfs:label>
    </owl:Class>
    


    <!-- http://purl.obolibrary.org/obo/GAZ_00619868 -->

    <owl:Class rdf:about="http://purl.obolibrary.org/obo/GAZ_00619868">
        <obo:IAO_0000115>A river.</obo:IAO_0000115>
        <oboInOwl:hasOBONamespace>GAZ</oboInOwl:hasOBONamespace>
        <oboInOwl:id>GAZ:00619868</oboInOwl:id>
        <rdfs:label>Hauptmunzkanal</rdfs:label>
    </owl:Class>
    


    <!-- http://purl.obolibrary.org/obo/GAZ_00619869 -->

    <owl:Class rdf:about="http://purl.obolibrary.org/obo/GAZ_00619869">
        <obo:IAO_0000115>A river.</obo:IAO_0000115>
        <oboInOwl:hasOBONamespace>GAZ</oboInOwl:hasOBONamespace>
        <oboInOwl:id>GAZ:00619869</oboInOwl:id>
        <rdfs:label>Hutfabrikkanal</rdfs:label>
    </owl:Class>
    


    <!-- http://purl.obolibrary.org/obo/GAZ_00619870 -->

    <owl:Class rdf:about="http://purl.obolibrary.org/obo/GAZ_00619870">
        <obo:IAO_0000115>A river.</obo:IAO_0000115>
        <oboInOwl:hasOBONamespace>GAZ</oboInOwl:hasOBONamespace>
        <oboInOwl:id>GAZ:00619870</oboInOwl:id>
        <rdfs:label>Kanalbachl</rdfs:label>
    </owl:Class>
    


    <!-- http://purl.obolibrary.org/obo/GAZ_00619871 -->

    <owl:Class rdf:about="http://purl.obolibrary.org/obo/GAZ_00619871">
        <obo:IAO_0000115>A river.</obo:IAO_0000115>
        <oboInOwl:hasOBONamespace>GAZ</oboInOwl:hasOBONamespace>
        <oboInOwl:id>GAZ:00619871</oboInOwl:id>
        <rdfs:label>Kaiblmuhlbach</rdfs:label>
    </owl:Class>
    


    <!-- http://purl.obolibrary.org/obo/GAZ_00619872 -->

    <owl:Class rdf:about="http://purl.obolibrary.org/obo/GAZ_00619872">
        <obo:IAO_0000115>A river.</obo:IAO_0000115>
        <oboInOwl:hasOBONamespace>GAZ</oboInOwl:hasOBONamespace>
        <oboInOwl:id>GAZ:00619872</oboInOwl:id>
        <rdfs:label>Kainzmuhlbach</rdfs:label>
    </owl:Class>
    


    <!-- http://purl.obolibrary.org/obo/GAZ_00619873 -->

    <owl:Class rdf:about="http://purl.obolibrary.org/obo/GAZ_00619873">
        <obo:IAO_0000115>A river.</obo:IAO_0000115>
        <oboInOwl:hasOBONamespace>GAZ</oboInOwl:hasOBONamespace>
        <oboInOwl:id>GAZ:00619873</oboInOwl:id>
        <rdfs:label>Kalblmuhlbach</rdfs:label>
    </owl:Class>
    


    <!-- http://purl.obolibrary.org/obo/GAZ_00619874 -->

    <owl:Class rdf:about="http://purl.obolibrary.org/obo/GAZ_00619874">
        <obo:IAO_0000115>A river.</obo:IAO_0000115>
        <oboInOwl:hasOBONamespace>GAZ</oboInOwl:hasOBONamespace>
        <oboInOwl:id>GAZ:00619874</oboInOwl:id>
        <rdfs:label>Kaltenbach</rdfs:label>
    </owl:Class>
    


    <!-- http://purl.obolibrary.org/obo/GAZ_00619875 -->

    <owl:Class rdf:about="http://purl.obolibrary.org/obo/GAZ_00619875">
        <obo:IAO_0000115>A river.</obo:IAO_0000115>
        <oboInOwl:hasOBONamespace>GAZ</oboInOwl:hasOBONamespace>
        <oboInOwl:id>GAZ:00619875</oboInOwl:id>
        <rdfs:label>Turkengraben</rdfs:label>
    </owl:Class>
    


    <!-- http://purl.obolibrary.org/obo/GAZ_00619877 -->

    <owl:Class rdf:about="http://purl.obolibrary.org/obo/GAZ_00619877">
        <obo:IAO_0000115>A river.</obo:IAO_0000115>
        <oboInOwl:hasOBONamespace>GAZ</oboInOwl:hasOBONamespace>
        <oboInOwl:id>GAZ:00619877</oboInOwl:id>
        <rdfs:label>Katzenbach</rdfs:label>
    </owl:Class>
    


    <!-- http://purl.obolibrary.org/obo/GAZ_00619878 -->

    <owl:Class rdf:about="http://purl.obolibrary.org/obo/GAZ_00619878">
        <obo:IAO_0000115>A river.</obo:IAO_0000115>
        <oboInOwl:hasOBONamespace>GAZ</oboInOwl:hasOBONamespace>
        <oboInOwl:id>GAZ:00619878</oboInOwl:id>
        <rdfs:label>Krankenhausbachl</rdfs:label>
    </owl:Class>
    


    <!-- http://purl.obolibrary.org/obo/GAZ_00619879 -->

    <owl:Class rdf:about="http://purl.obolibrary.org/obo/GAZ_00619879">
        <obo:IAO_0000115>A river.</obo:IAO_0000115>
        <oboInOwl:hasOBONamespace>GAZ</oboInOwl:hasOBONamespace>
        <oboInOwl:id>GAZ:00619879</oboInOwl:id>
        <rdfs:label>Laimbach</rdfs:label>
    </owl:Class>
    


    <!-- http://purl.obolibrary.org/obo/GAZ_00619880 -->

    <owl:Class rdf:about="http://purl.obolibrary.org/obo/GAZ_00619880">
        <obo:IAO_0000115>A river.</obo:IAO_0000115>
        <oboInOwl:hasOBONamespace>GAZ</oboInOwl:hasOBONamespace>
        <oboInOwl:id>GAZ:00619880</oboInOwl:id>
        <rdfs:label>Lazarettbach</rdfs:label>
    </owl:Class>
    


    <!-- http://purl.obolibrary.org/obo/GAZ_00619881 -->

    <owl:Class rdf:about="http://purl.obolibrary.org/obo/GAZ_00619881">
        <obo:IAO_0000115>A river.</obo:IAO_0000115>
        <oboInOwl:hasOBONamespace>GAZ</oboInOwl:hasOBONamespace>
        <oboInOwl:id>GAZ:00619881</oboInOwl:id>
        <rdfs:label>Malzmuhlbach</rdfs:label>
    </owl:Class>
    


    <!-- http://purl.obolibrary.org/obo/GAZ_00619882 -->

    <owl:Class rdf:about="http://purl.obolibrary.org/obo/GAZ_00619882">
        <obo:IAO_0000115>A river.</obo:IAO_0000115>
        <oboInOwl:hasOBONamespace>GAZ</oboInOwl:hasOBONamespace>
        <oboInOwl:id>GAZ:00619882</oboInOwl:id>
        <rdfs:label>Munzbachl</rdfs:label>
    </owl:Class>
    


    <!-- http://purl.obolibrary.org/obo/GAZ_00619883 -->

    <owl:Class rdf:about="http://purl.obolibrary.org/obo/GAZ_00619883">
        <obo:IAO_0000115>A river.</obo:IAO_0000115>
        <oboInOwl:hasOBONamespace>GAZ</oboInOwl:hasOBONamespace>
        <oboInOwl:id>GAZ:00619883</oboInOwl:id>
        <rdfs:label>Muffatbrunnhauskanal</rdfs:label>
    </owl:Class>
    


    <!-- http://purl.obolibrary.org/obo/GAZ_00619885 -->

    <owl:Class rdf:about="http://purl.obolibrary.org/obo/GAZ_00619885">
        <obo:IAO_0000115>A river.</obo:IAO_0000115>
        <oboInOwl:hasOBONamespace>GAZ</oboInOwl:hasOBONamespace>
        <oboInOwl:id>GAZ:00619885</oboInOwl:id>
        <rdfs:label>Papiererbach</rdfs:label>
    </owl:Class>
    


    <!-- http://purl.obolibrary.org/obo/GAZ_00619886 -->

    <owl:Class rdf:about="http://purl.obolibrary.org/obo/GAZ_00619886">
        <obo:IAO_0000115>A river.</obo:IAO_0000115>
        <oboInOwl:hasOBONamespace>GAZ</oboInOwl:hasOBONamespace>
        <oboInOwl:id>GAZ:00619886</oboInOwl:id>
        <rdfs:label>Palaisbachl</rdfs:label>
    </owl:Class>
    


    <!-- http://purl.obolibrary.org/obo/GAZ_00619887 -->

    <owl:Class rdf:about="http://purl.obolibrary.org/obo/GAZ_00619887">
        <obo:IAO_0000115>A river.</obo:IAO_0000115>
        <oboInOwl:hasOBONamespace>GAZ</oboInOwl:hasOBONamespace>
        <oboInOwl:id>GAZ:00619887</oboInOwl:id>
        <rdfs:label>Pfisterbach</rdfs:label>
    </owl:Class>
    


    <!-- http://purl.obolibrary.org/obo/GAZ_00619888 -->

    <owl:Class rdf:about="http://purl.obolibrary.org/obo/GAZ_00619888">
        <obo:IAO_0000115>A river.</obo:IAO_0000115>
        <oboInOwl:hasOBONamespace>GAZ</oboInOwl:hasOBONamespace>
        <oboInOwl:id>GAZ:00619888</oboInOwl:id>
        <rdfs:label>Rossschwemmbach</rdfs:label>
    </owl:Class>
    


    <!-- http://purl.obolibrary.org/obo/GAZ_00619889 -->

    <owl:Class rdf:about="http://purl.obolibrary.org/obo/GAZ_00619889">
        <obo:IAO_0000115>A river.</obo:IAO_0000115>
        <oboInOwl:hasOBONamespace>GAZ</oboInOwl:hasOBONamespace>
        <oboInOwl:id>GAZ:00619889</oboInOwl:id>
        <rdfs:label>Stadthammerschmiedbach</rdfs:label>
    </owl:Class>
    


    <!-- http://purl.obolibrary.org/obo/GAZ_00619890 -->

    <owl:Class rdf:about="http://purl.obolibrary.org/obo/GAZ_00619890">
        <obo:IAO_0000115>A river.</obo:IAO_0000115>
        <oboInOwl:hasOBONamespace>GAZ</oboInOwl:hasOBONamespace>
        <oboInOwl:id>GAZ:00619890</oboInOwl:id>
        <rdfs:label>Steinsagkanal</rdfs:label>
    </owl:Class>
    


    <!-- http://purl.obolibrary.org/obo/GAZ_00619891 -->

    <owl:Class rdf:about="http://purl.obolibrary.org/obo/GAZ_00619891">
        <obo:IAO_0000115>A river.</obo:IAO_0000115>
        <oboInOwl:hasOBONamespace>GAZ</oboInOwl:hasOBONamespace>
        <oboInOwl:id>GAZ:00619891</oboInOwl:id>
        <rdfs:label>Strihhannerbach</rdfs:label>
    </owl:Class>
    


    <!-- http://purl.obolibrary.org/obo/GAZ_00619892 -->

    <owl:Class rdf:about="http://purl.obolibrary.org/obo/GAZ_00619892">
        <obo:IAO_0000115>A river.</obo:IAO_0000115>
        <oboInOwl:hasOBONamespace>GAZ</oboInOwl:hasOBONamespace>
        <oboInOwl:id>GAZ:00619892</oboInOwl:id>
        <rdfs:label>Stadtmuhlbach</rdfs:label>
    </owl:Class>
    


    <!-- http://purl.obolibrary.org/obo/GAZ_00619893 -->

    <owl:Class rdf:about="http://purl.obolibrary.org/obo/GAZ_00619893">
        <obo:IAO_0000115>A river.</obo:IAO_0000115>
        <oboInOwl:hasOBONamespace>GAZ</oboInOwl:hasOBONamespace>
        <oboInOwl:id>GAZ:00619893</oboInOwl:id>
        <rdfs:label>Stadtsagmuhlbach</rdfs:label>
    </owl:Class>
    


    <!-- http://purl.obolibrary.org/obo/GAZ_00619894 -->

    <owl:Class rdf:about="http://purl.obolibrary.org/obo/GAZ_00619894">
        <obo:IAO_0000115>A river.</obo:IAO_0000115>
        <oboInOwl:hasOBONamespace>GAZ</oboInOwl:hasOBONamespace>
        <oboInOwl:id>GAZ:00619894</oboInOwl:id>
        <rdfs:label>Triftkanal</rdfs:label>
    </owl:Class>
    


    <!-- http://purl.obolibrary.org/obo/GAZ_00619895 -->

    <owl:Class rdf:about="http://purl.obolibrary.org/obo/GAZ_00619895">
        <obo:IAO_0000115>A river.</obo:IAO_0000115>
        <oboInOwl:hasOBONamespace>GAZ</oboInOwl:hasOBONamespace>
        <oboInOwl:id>GAZ:00619895</oboInOwl:id>
        <rdfs:label>Triftkanal-Auslaufer</rdfs:label>
    </owl:Class>
    


    <!-- http://purl.obolibrary.org/obo/GAZ_00619896 -->

    <owl:Class rdf:about="http://purl.obolibrary.org/obo/GAZ_00619896">
        <obo:IAO_0000115>A river.</obo:IAO_0000115>
        <oboInOwl:hasOBONamespace>GAZ</oboInOwl:hasOBONamespace>
        <oboInOwl:id>GAZ:00619896</oboInOwl:id>
        <rdfs:label>Wuhrbach</rdfs:label>
    </owl:Class>
    


    <!-- http://purl.obolibrary.org/obo/GAZ_00658555 -->

    <owl:Class rdf:about="http://purl.obolibrary.org/obo/GAZ_00658555">
        <oboInOwl:hasOBONamespace>GAZ</oboInOwl:hasOBONamespace>
        <oboInOwl:id>GAZ:00658555</oboInOwl:id>
        <rdfs:label>Seebach</rdfs:label>
    </owl:Class>
    


    <!-- 
    ///////////////////////////////////////////////////////////////////////////////////////
    //
    // Individuals
    //
    ///////////////////////////////////////////////////////////////////////////////////////
     -->

    


    <!-- http://purl.obolibrary.org/obo/GAZ_00003858 -->

    <owl:NamedIndividual rdf:about="http://purl.obolibrary.org/obo/GAZ_00003858">
        <obo:IAO_0000115>A tiny, doubly landlocked alpine country in Western Europe, bordered by Switzerland to its west and by Austria to its east. The principality of Liechtenstein is divided into 11 municipalities called Gemeinden (singular Gemeinde). The Gemeinden mostly consist only of a single town. Five of them fall within the electoral district Unterland (the lower county), and the remainder within Oberland (the upper county).</obo:IAO_0000115>
        <oboInOwl:hasOBONamespace>GAZ</oboInOwl:hasOBONamespace>
        <oboInOwl:id>GAZ:00003858</oboInOwl:id>
        <rdfs:label>Liechtenstein</rdfs:label>
    </owl:NamedIndividual>
    


    <!-- http://purl.obolibrary.org/obo/GAZ_00004122 -->

    <owl:NamedIndividual rdf:about="http://purl.obolibrary.org/obo/GAZ_00004122">
        <obo:RO_0001025 rdf:resource="http://purl.obolibrary.org/obo/GAZ_00051915"/>
        <obo:IAO_0000115>Ein Berg in den Nordlichen Kalkalpen an der steirisch-niederosterreichischen Grenze.</obo:IAO_0000115>
        <oboInOwl:hasOBONamespace>GAZ</oboInOwl:hasOBONamespace>
        <oboInOwl:id>GAZ:00004122</oboInOwl:id>
        <rdfs:label>Schneealpe</rdfs:label>
    </owl:NamedIndividual>
    


    <!-- http://purl.obolibrary.org/obo/GAZ_00004124 -->

    <owl:NamedIndividual rdf:about="http://purl.obolibrary.org/obo/GAZ_00004124">
        <obo:RO_0001025 rdf:resource="http://purl.obolibrary.org/obo/GAZ_00051915"/>
        <obo:IAO_0000115>A low, wooded section of the Alps in eastern Lower Austria and Vienna, covering over 1,000 km2 and including the northernmost parts of the entire Alpine chain. The Vienna Woods may be defined as that group of hills bounded by the rivers Triesting, Golsen, Traisen and Danube.</obo:IAO_0000115>
        <oboInOwl:hasOBONamespace>GAZ</oboInOwl:hasOBONamespace>
        <oboInOwl:id>GAZ:00004124</oboInOwl:id>
        <rdfs:label>Wienerwald</rdfs:label>
    </owl:NamedIndividual>
    


    <!-- http://purl.obolibrary.org/obo/GAZ_00005321 -->

    <owl:NamedIndividual rdf:about="http://purl.obolibrary.org/obo/GAZ_00005321">
        <obo:RO_0001025 rdf:resource="http://purl.obolibrary.org/obo/GAZ_00009680"/>
        <oboInOwl:hasOBONamespace>GAZ</oboInOwl:hasOBONamespace>
        <oboInOwl:id>GAZ:00005321</oboInOwl:id>
        <rdfs:label>Saint Gothard Pass</rdfs:label>
    </owl:NamedIndividual>
    


    <!-- http://purl.obolibrary.org/obo/GAZ_00005367 -->

    <owl:NamedIndividual rdf:about="http://purl.obolibrary.org/obo/GAZ_00005367">
        <obo:RO_0001025 rdf:resource="http://purl.obolibrary.org/obo/GAZ_00012576"/>
    </owl:NamedIndividual>
    


    <!-- http://purl.obolibrary.org/obo/GAZ_00005544 -->

    <owl:NamedIndividual rdf:about="http://purl.obolibrary.org/obo/GAZ_00005544">
        <obo:RO_0001025 rdf:resource="http://purl.obolibrary.org/obo/GAZ_00012545"/>
    </owl:NamedIndividual>
    


    <!-- http://purl.obolibrary.org/obo/GAZ_00006569 -->

    <owl:NamedIndividual rdf:about="http://purl.obolibrary.org/obo/GAZ_00006569">
        <obo:RO_0001025 rdf:resource="http://purl.obolibrary.org/obo/GAZ_00060601"/>
        <obo:IAO_0000115>A mountain ridge spreading between the Departments of Bouches-du-Rhone and Var in southern France.</obo:IAO_0000115>
        <oboInOwl:hasOBONamespace>GAZ</oboInOwl:hasOBONamespace>
        <oboInOwl:id>GAZ:00006569</oboInOwl:id>
        <rdfs:label>Massif de la Sainte-Baume</rdfs:label>
    </owl:NamedIndividual>
    


    <!-- http://purl.obolibrary.org/obo/GAZ_00006787 -->

    <owl:NamedIndividual rdf:about="http://purl.obolibrary.org/obo/GAZ_00006787">
        <obo:RO_0001025 rdf:resource="http://purl.obolibrary.org/obo/GAZ_00060601"/>
        <obo:IAO_0000115>Un massif des Prealpes situe dans le sud de la France, a cheval sur les departements du Vaucluse et des Alpes-de-Haute-Provence, a 70 km au nord de Marseille. Il s&apos;etend sur 60 km d&apos;est en ouest pour 5 km de largeur moyenne. Il est limite par le Calavon et les monts de Vaucluse au nord et la Durance au sud.</obo:IAO_0000115>
        <oboInOwl:hasOBONamespace>GAZ</oboInOwl:hasOBONamespace>
        <oboInOwl:id>GAZ:00006787</oboInOwl:id>
        <rdfs:label>Massif du Luberon</rdfs:label>
    </owl:NamedIndividual>
    


    <!-- http://purl.obolibrary.org/obo/GAZ_00007412 -->

    <owl:NamedIndividual rdf:about="http://purl.obolibrary.org/obo/GAZ_00007412">
        <obo:RO_0001025 rdf:resource="http://purl.obolibrary.org/obo/GAZ_00012567"/>
    </owl:NamedIndividual>
    


    <!-- http://purl.obolibrary.org/obo/GAZ_00008018 -->

    <owl:NamedIndividual rdf:about="http://purl.obolibrary.org/obo/GAZ_00008018">
        <obo:RO_0001025 rdf:resource="http://purl.obolibrary.org/obo/GAZ_00060601"/>
        <obo:IAO_0000115>Un massif montagneux situe au nord-ouest du departement des Bouches-du-Rhone. Les Alpilles s&apos;etendent selon un axe est-ouest sur environ 25 km, depuis la vallee du Rhone jusqu&apos;a la vallee de la Durance. Il domine au nord la plaine maraichere de Saint-Remy-de-Provence et au sud la plaine de la Crau.</obo:IAO_0000115>
        <oboInOwl:hasOBONamespace>GAZ</oboInOwl:hasOBONamespace>
        <oboInOwl:id>GAZ:00008018</oboInOwl:id>
        <rdfs:label>Chaine des Alpilles</rdfs:label>
    </owl:NamedIndividual>
    


    <!-- http://purl.obolibrary.org/obo/GAZ_00008019 -->

    <owl:NamedIndividual rdf:about="http://purl.obolibrary.org/obo/GAZ_00008019">
        <obo:RO_0001025 rdf:resource="http://purl.obolibrary.org/obo/GAZ_00008018"/>
        <obo:IAO_0000115>A archeological site. Une cite antique de l&apos;empire romain situee pres du village de Saint-Remy de Provence dans les Bouches-du-Rhone.</obo:IAO_0000115>
        <oboInOwl:hasOBONamespace>GAZ</oboInOwl:hasOBONamespace>
        <oboInOwl:id>GAZ:00008019</oboInOwl:id>
        <rdfs:label>Les Antiques</rdfs:label>
    </owl:NamedIndividual>
    


    <!-- http://purl.obolibrary.org/obo/GAZ_00008111 -->

    <owl:NamedIndividual rdf:about="http://purl.obolibrary.org/obo/GAZ_00008111">
        <obo:RO_0001025 rdf:resource="http://purl.obolibrary.org/obo/GAZ_00008262"/>
        <obo:IAO_0000115>A large monomictic lake on the Rhine between Germany, Switzerland, and Austria. The regulated Rhine flows into the lake in the southeast, through the Obersee, the city of Konstanz and the Untersee and flows out near Stein am Rhein.</obo:IAO_0000115>
        <oboInOwl:hasOBONamespace>GAZ</oboInOwl:hasOBONamespace>
        <oboInOwl:id>GAZ:00008111</oboInOwl:id>
        <rdfs:label>Bodensee</rdfs:label>
    </owl:NamedIndividual>
    


    <!-- http://purl.obolibrary.org/obo/GAZ_00008197 -->

    <owl:NamedIndividual rdf:about="http://purl.obolibrary.org/obo/GAZ_00008197">
        <obo:RO_0001025 rdf:resource="http://purl.obolibrary.org/obo/GAZ_00008200"/>
        <obo:IAO_0000115>The highest mountain in the Graian Alps, is located in the Aosta Valley region of north-west Italy.</obo:IAO_0000115>
        <oboInOwl:hasOBONamespace>GAZ</oboInOwl:hasOBONamespace>
        <oboInOwl:id>GAZ:00008197</oboInOwl:id>
        <rdfs:label>Gran Paradiso</rdfs:label>
    </owl:NamedIndividual>
    


    <!-- http://purl.obolibrary.org/obo/GAZ_00008198 -->

    <owl:NamedIndividual rdf:about="http://purl.obolibrary.org/obo/GAZ_00008198">
        <obo:RO_0001025 rdf:resource="http://purl.obolibrary.org/obo/GAZ_00008197"/>
        <obo:IAO_0000115>A populated place. A hamlet in the Commune of Cogne.</obo:IAO_0000115>
        <oboInOwl:hasOBONamespace>GAZ</oboInOwl:hasOBONamespace>
        <oboInOwl:id>GAZ:00008198</oboInOwl:id>
        <rdfs:label>Valnontey</rdfs:label>
    </owl:NamedIndividual>
    


    <!-- http://purl.obolibrary.org/obo/GAZ_00008200 -->

    <owl:NamedIndividual rdf:about="http://purl.obolibrary.org/obo/GAZ_00008200">
        <obo:RO_0001025 rdf:resource="http://purl.obolibrary.org/obo/GAZ_00051917"/>
        <obo:IAO_0000115>A mountain range in the western part of the Alps. They are located in France (Savoie), Italy (Piedmont and the Aosta Valley), and Switzerland (western Valais). The Col Ferret and the Dora Baltea valley separate them from the Pennine Alps; the Col du Mont Cenis separates them from the Cottian Alps; the Arc valley separates them from the Dauphine Alps; the Chablais mountains lie to the northwest.</obo:IAO_0000115>
        <oboInOwl:hasOBONamespace>GAZ</oboInOwl:hasOBONamespace>
        <oboInOwl:id>GAZ:00008200</oboInOwl:id>
        <rdfs:label>Graian Alps</rdfs:label>
    </owl:NamedIndividual>
    


    <!-- http://purl.obolibrary.org/obo/GAZ_00008249 -->

    <owl:NamedIndividual rdf:about="http://purl.obolibrary.org/obo/GAZ_00008249">
        <obo:IAO_0000115>A 367-km long river, mainly flowing through the southwestern State of Baden-Wurttemberg, but also a short section through Hesse in Germany, a major right tributary of the River Rhine, which it joins at Mannheim.</obo:IAO_0000115>
        <oboInOwl:hasOBONamespace>GAZ</oboInOwl:hasOBONamespace>
        <oboInOwl:id>GAZ:00008249</oboInOwl:id>
        <rdfs:label>Neckar</rdfs:label>
    </owl:NamedIndividual>
    


    <!-- http://purl.obolibrary.org/obo/GAZ_00008262 -->

    <owl:NamedIndividual rdf:about="http://purl.obolibrary.org/obo/GAZ_00008262"/>
    


    <!-- http://purl.obolibrary.org/obo/GAZ_00008403 -->

    <owl:NamedIndividual rdf:about="http://purl.obolibrary.org/obo/GAZ_00008403">
        <obo:RO_0001025 rdf:resource="http://purl.obolibrary.org/obo/GAZ_00060609"/>
        <obo:IAO_0000115>A mountain range in the western part of the Alps. They are located in Switzerland (Valais) and Italy (Piedmont and the Aosta Valley). The Col Ferret separates them from the Mont Blanc Massif; the Dora Baltea valley separates them from the Graian Alps; the Simplon Pass separates them from the Lepontine Alps; the Rhone valley separates them from the Bernese Alps. The Italian side is drained by the rivers Dora Baltea, Sesia and Toce, tributaries of the Po. The Swiss side is drained by the Rhone River.</obo:IAO_0000115>
        <oboInOwl:hasOBONamespace>GAZ</oboInOwl:hasOBONamespace>
        <oboInOwl:id>GAZ:00008403</oboInOwl:id>
        <rdfs:label>Pennine Alps</rdfs:label>
    </owl:NamedIndividual>
    


    <!-- http://purl.obolibrary.org/obo/GAZ_00008405 -->

    <owl:NamedIndividual rdf:about="http://purl.obolibrary.org/obo/GAZ_00008405">
        <obo:RO_0001025 rdf:resource="http://purl.obolibrary.org/obo/GAZ_00051917"/>
        <obo:IAO_0000115>A mountain range in the south-western part of the Alps. They form the border between France (Hautes-Alpes and Savoie) and Italy (Piedmont). The Maddalena Pass separates them from the Maritime Alps; the Col du Mont Cenis separates them from the Graian Alps; the Col du Galibier separates them from the Dauphine Alps. The Cottian Alps are drained by the rivers Durance and Arc and their tributaries on the French side; by the Dora Riparia and other tributaries of the Po on the Italian side.</obo:IAO_0000115>
        <oboInOwl:hasOBONamespace>GAZ</oboInOwl:hasOBONamespace>
        <oboInOwl:id>GAZ:00008405</oboInOwl:id>
        <rdfs:label>Cottian Alps</rdfs:label>
    </owl:NamedIndividual>
    


    <!-- http://purl.obolibrary.org/obo/GAZ_00008406 -->

    <owl:NamedIndividual rdf:about="http://purl.obolibrary.org/obo/GAZ_00008406">
        <obo:RO_0001025 rdf:resource="http://purl.obolibrary.org/obo/GAZ_00051917"/>
        <obo:IAO_0000115>A mountain range in Italy. They form the south-western extremity of the Alps, separated from the Apennines by the Colle di Cadibona. The Col de Tende separates them from the Maritime Alps. They form the border between Piedmont in the north and Liguria in the south. The Ligurian Alps are drained by the river Tanaro and other tributaries of the Po on the Piemontese side; by several smaller rivers that flow directly to the Mediterranean Sea on the Ligurian side.</obo:IAO_0000115>
        <oboInOwl:hasOBONamespace>GAZ</oboInOwl:hasOBONamespace>
        <oboInOwl:id>GAZ:00008406</oboInOwl:id>
        <rdfs:label>Ligurian Alps</rdfs:label>
    </owl:NamedIndividual>
    


    <!-- http://purl.obolibrary.org/obo/GAZ_00008474 -->

    <owl:NamedIndividual rdf:about="http://purl.obolibrary.org/obo/GAZ_00008474">
        <obo:RO_0001025 rdf:resource="http://purl.obolibrary.org/obo/GAZ_00009680"/>
        <obo:IAO_0000115>A canyon around 5 km long on the Reuss River in central Switzerland north of Andermatt.</obo:IAO_0000115>
        <oboInOwl:hasOBONamespace>GAZ</oboInOwl:hasOBONamespace>
        <oboInOwl:id>GAZ:00008474</oboInOwl:id>
        <rdfs:label>Schollenen Gorge</rdfs:label>
    </owl:NamedIndividual>
    


    <!-- http://purl.obolibrary.org/obo/GAZ_00008475 -->

    <owl:NamedIndividual rdf:about="http://purl.obolibrary.org/obo/GAZ_00008475">
        <obo:RO_0001025 rdf:resource="http://purl.obolibrary.org/obo/GAZ_00008474"/>
        <oboInOwl:hasOBONamespace>GAZ</oboInOwl:hasOBONamespace>
        <oboInOwl:id>GAZ:00008475</oboInOwl:id>
        <rdfs:label>Teufelsbrucke</rdfs:label>
    </owl:NamedIndividual>
    


    <!-- http://purl.obolibrary.org/obo/GAZ_00009543 -->

    <owl:NamedIndividual rdf:about="http://purl.obolibrary.org/obo/GAZ_00009543">
        <obo:RO_0001025 rdf:resource="http://purl.obolibrary.org/obo/GAZ_00003858"/>
    </owl:NamedIndividual>
    


    <!-- http://purl.obolibrary.org/obo/GAZ_00009674 -->

    <owl:NamedIndividual rdf:about="http://purl.obolibrary.org/obo/GAZ_00009674">
        <obo:RO_0001025 rdf:resource="http://purl.obolibrary.org/obo/GAZ_00060609"/>
        <obo:IAO_0000115>A mountain range in central Switzerland. They extend from the Oberalp Pass to the Klausen Pass, and are bordered by the Urner Alps to the west, the Lepontine Alps to the south and the Appenzell Alps to the north-east.</obo:IAO_0000115>
        <oboInOwl:hasOBONamespace>GAZ</oboInOwl:hasOBONamespace>
        <oboInOwl:id>GAZ:00009674</oboInOwl:id>
        <rdfs:label>Glarus Alps</rdfs:label>
    </owl:NamedIndividual>
    


    <!-- http://purl.obolibrary.org/obo/GAZ_00009675 -->

    <owl:NamedIndividual rdf:about="http://purl.obolibrary.org/obo/GAZ_00009675">
        <obo:RO_0001025 rdf:resource="http://purl.obolibrary.org/obo/GAZ_00051917"/>
        <obo:IAO_0000115>A group of mountain ranges in southeastern France, west of the main chain of the Alps. They are separated from the Cottian Alps in the east by the Col du Galibier and the upper Durance valley; from the western Graian Alps (Vanoise) in the north-east by the river Arc; from the lower ranges Vercors Plateau and Chartreuse Mountains in the west by the rivers Drac and Isere.</obo:IAO_0000115>
        <oboInOwl:hasOBONamespace>GAZ</oboInOwl:hasOBONamespace>
        <oboInOwl:id>GAZ:00009675</oboInOwl:id>
        <rdfs:label>Dauphine Alps</rdfs:label>
    </owl:NamedIndividual>
    


    <!-- http://purl.obolibrary.org/obo/GAZ_00009676 -->

    <owl:NamedIndividual rdf:about="http://purl.obolibrary.org/obo/GAZ_00009676">
        <obo:RO_0001025 rdf:resource="http://purl.obolibrary.org/obo/GAZ_00060609"/>
        <obo:IAO_0000115>A group of mountain ranges in the western part of the Alps, in Switzerland. The Rhone valley separates it from the Pennine Alps in the south; the Furka Pass, Saint Gotthard Pass and the upper Rhone valley separate it from the Lepontine Alps in the south-east; the Reuss valley separates it from the Glarus Alps in the east; the northern edge is not so well defined, roughly a line from Lake Geneva to Lake Lucerne. The Bernese Alps are drained by the river Aar and its tributary Saane in the north, the Rhone in the south and the Reuss in the east.</obo:IAO_0000115>
        <oboInOwl:hasOBONamespace>GAZ</oboInOwl:hasOBONamespace>
        <oboInOwl:id>GAZ:00009676</oboInOwl:id>
        <rdfs:label>Bernese Alps</rdfs:label>
    </owl:NamedIndividual>
    


    <!-- http://purl.obolibrary.org/obo/GAZ_00009677 -->

    <owl:NamedIndividual rdf:about="http://purl.obolibrary.org/obo/GAZ_00009677">
        <obo:RO_0001025 rdf:resource="http://purl.obolibrary.org/obo/GAZ_00051917"/>
        <obo:IAO_0000115>The part of the Alps and Pre-Alps that is located in North-Eastern Switzerland. This region is bordered by: Lake Lucerne in the south-west; the Klausen Pass, upper Linth valley and Lake Walen in the south; the Rhine valley in the east; Lake Constance in the north.</obo:IAO_0000115>
        <oboInOwl:hasOBONamespace>GAZ</oboInOwl:hasOBONamespace>
        <oboInOwl:id>GAZ:00009677</oboInOwl:id>
        <rdfs:label>North-Eastern Swiss Alps</rdfs:label>
    </owl:NamedIndividual>
    


    <!-- http://purl.obolibrary.org/obo/GAZ_00009679 -->

    <owl:NamedIndividual rdf:about="http://purl.obolibrary.org/obo/GAZ_00009679">
        <obo:RO_0001025 rdf:resource="http://purl.obolibrary.org/obo/GAZ_00051917"/>
        <obo:IAO_0000115>A mountain range in the south-western part of the Alps. They form the border between the French departement Alpes-Maritimes and the Italian province of Cuneo. The Col de Tende separates them from the Ligurian Alps; the Maddalena Pass separates them from the Cottian Alps. The Maritime Alps are drained by the rivers Roya, Var and Verdon and their tributaries on the French side; by the Stura di Demonte and other tributaries of the Tanaro and Po on the Italian side.</obo:IAO_0000115>
        <oboInOwl:hasOBONamespace>GAZ</oboInOwl:hasOBONamespace>
        <oboInOwl:id>GAZ:00009679</oboInOwl:id>
        <rdfs:label>Maritime Alps</rdfs:label>
    </owl:NamedIndividual>
    


    <!-- http://purl.obolibrary.org/obo/GAZ_00009680 -->

    <owl:NamedIndividual rdf:about="http://purl.obolibrary.org/obo/GAZ_00009680">
        <obo:RO_0001025 rdf:resource="http://purl.obolibrary.org/obo/GAZ_00060609"/>
        <obo:IAO_0000115>A mountain range in the central part of the Alps. They are located in Switzerland (Valais, Ticino and Graubunden) and Italy (Piedmont). The Furka Pass, St Gotthard Pass and the upper Rhone valley separate them from the Bernese Alps; the Simplon Pass separates them from the Pennine Alps; the Vorderrhein valley and the Oberalp Pass separate them from the Glarus Alps; the Splugen Pass separates them from the Central Eastern Alps (Oberhalbstein Range). The Lepontine Alps are drained by the rivers Rhone in the west, Reuss in the north, Rhine (Vorderrhein and Hinterrhein) in the east and Ticino and Toce in the south.</obo:IAO_0000115>
        <oboInOwl:hasOBONamespace>GAZ</oboInOwl:hasOBONamespace>
        <oboInOwl:id>GAZ:00009680</oboInOwl:id>
        <rdfs:label>Lepontine Alps</rdfs:label>
    </owl:NamedIndividual>
    


    <!-- http://purl.obolibrary.org/obo/GAZ_00011833 -->

    <owl:NamedIndividual rdf:about="http://purl.obolibrary.org/obo/GAZ_00011833">
        <obo:RO_0001025 rdf:resource="http://purl.obolibrary.org/obo/GAZ_00058617"/>
        <obo:IAO_0000115>A land-tied island.</obo:IAO_0000115>
        <oboInOwl:hasOBONamespace>GAZ</oboInOwl:hasOBONamespace>
        <oboInOwl:id>GAZ:00011833</oboInOwl:id>
        <rdfs:label>Mainau</rdfs:label>
    </owl:NamedIndividual>
    


    <!-- http://purl.obolibrary.org/obo/GAZ_00012396 -->

    <owl:NamedIndividual rdf:about="http://purl.obolibrary.org/obo/GAZ_00012396">
        <obo:RO_0001025 rdf:resource="http://purl.obolibrary.org/obo/GAZ_00060642"/>
        <obo:IAO_0000115>A dimictic lake in the Salzkammergut area of Austria. It extends for about 20 km from north to south and 4 km from east to west Its water comes from the Seeache, which flows out of another lake, the Mondsee.</obo:IAO_0000115>
        <oboInOwl:hasOBONamespace>GAZ</oboInOwl:hasOBONamespace>
        <oboInOwl:id>GAZ:00012396</oboInOwl:id>
        <rdfs:label>Attersee</rdfs:label>
    </owl:NamedIndividual>
    


    <!-- http://purl.obolibrary.org/obo/GAZ_00012545 -->

    <owl:NamedIndividual rdf:about="http://purl.obolibrary.org/obo/GAZ_00012545">
        <rdf:type rdf:resource="http://purl.obolibrary.org/obo/ENVO_00000856"/>
        <obo:RO_0001025 rdf:resource="http://purl.obolibrary.org/obo/GAZ_00144362"/>
        <obo:IAO_0000115>A municipality.</obo:IAO_0000115>
        <oboInOwl:hasOBONamespace>GAZ</oboInOwl:hasOBONamespace>
        <oboInOwl:id>GAZ:00012545</oboInOwl:id>
        <rdfs:label>Municipality of Goes</rdfs:label>
    </owl:NamedIndividual>
    


    <!-- http://purl.obolibrary.org/obo/GAZ_00012567 -->

    <owl:NamedIndividual rdf:about="http://purl.obolibrary.org/obo/GAZ_00012567">
        <rdf:type rdf:resource="http://purl.obolibrary.org/obo/ENVO_00000856"/>
        <obo:RO_0001025 rdf:resource="http://purl.obolibrary.org/obo/GAZ_00043990"/>
        <obo:IAO_0000115>A municipality.</obo:IAO_0000115>
        <oboInOwl:hasOBONamespace>GAZ</oboInOwl:hasOBONamespace>
        <oboInOwl:id>GAZ:00012567</oboInOwl:id>
        <rdfs:label>Municipality of Zwijndrecht</rdfs:label>
    </owl:NamedIndividual>
    


    <!-- http://purl.obolibrary.org/obo/GAZ_00012576 -->

    <owl:NamedIndividual rdf:about="http://purl.obolibrary.org/obo/GAZ_00012576">
        <rdf:type rdf:resource="http://purl.obolibrary.org/obo/ENVO_00000856"/>
        <obo:RO_0001025 rdf:resource="http://purl.obolibrary.org/obo/GAZ_00144371"/>
        <obo:IAO_0000115>A municipality.</obo:IAO_0000115>
        <oboInOwl:hasOBONamespace>GAZ</oboInOwl:hasOBONamespace>
        <oboInOwl:id>GAZ:00012576</oboInOwl:id>
        <rdfs:label>Municipality of Veere</rdfs:label>
    </owl:NamedIndividual>
    


    <!-- http://purl.obolibrary.org/obo/GAZ_00013805 -->

    <owl:NamedIndividual rdf:about="http://purl.obolibrary.org/obo/GAZ_00013805"/>
    


    <!-- http://purl.obolibrary.org/obo/GAZ_00013807 -->

    <owl:NamedIndividual rdf:about="http://purl.obolibrary.org/obo/GAZ_00013807"/>
    


    <!-- http://purl.obolibrary.org/obo/GAZ_00013808 -->

    <owl:NamedIndividual rdf:about="http://purl.obolibrary.org/obo/GAZ_00013808"/>
    


    <!-- http://purl.obolibrary.org/obo/GAZ_00013809 -->

    <owl:NamedIndividual rdf:about="http://purl.obolibrary.org/obo/GAZ_00013809"/>
    


    <!-- http://purl.obolibrary.org/obo/GAZ_00013810 -->

    <owl:NamedIndividual rdf:about="http://purl.obolibrary.org/obo/GAZ_00013810"/>
    


    <!-- http://purl.obolibrary.org/obo/GAZ_00013811 -->

    <owl:NamedIndividual rdf:about="http://purl.obolibrary.org/obo/GAZ_00013811"/>
    


    <!-- http://purl.obolibrary.org/obo/GAZ_00013812 -->

    <owl:NamedIndividual rdf:about="http://purl.obolibrary.org/obo/GAZ_00013812"/>
    


    <!-- http://purl.obolibrary.org/obo/GAZ_00013813 -->

    <owl:NamedIndividual rdf:about="http://purl.obolibrary.org/obo/GAZ_00013813"/>
    


    <!-- http://purl.obolibrary.org/obo/GAZ_00013814 -->

    <owl:NamedIndividual rdf:about="http://purl.obolibrary.org/obo/GAZ_00013814"/>
    


    <!-- http://purl.obolibrary.org/obo/GAZ_00013815 -->

    <owl:NamedIndividual rdf:about="http://purl.obolibrary.org/obo/GAZ_00013815"/>
    


    <!-- http://purl.obolibrary.org/obo/GAZ_00013816 -->

    <owl:NamedIndividual rdf:about="http://purl.obolibrary.org/obo/GAZ_00013816">
        <obo:RO_0001025 rdf:resource="http://purl.obolibrary.org/obo/GAZ_00013814"/>
    </owl:NamedIndividual>
    


    <!-- http://purl.obolibrary.org/obo/GAZ_00013817 -->

    <owl:NamedIndividual rdf:about="http://purl.obolibrary.org/obo/GAZ_00013817">
        <obo:RO_0001025 rdf:resource="http://purl.obolibrary.org/obo/GAZ_00003858"/>
    </owl:NamedIndividual>
    


    <!-- http://purl.obolibrary.org/obo/GAZ_00015662 -->

    <owl:NamedIndividual rdf:about="http://purl.obolibrary.org/obo/GAZ_00015662">
        <obo:RO_0001025 rdf:resource="http://purl.obolibrary.org/obo/GAZ_00056798"/>
        <oboInOwl:hasOBONamespace>GAZ</oboInOwl:hasOBONamespace>
        <oboInOwl:id>GAZ:00015662</oboInOwl:id>
        <rdfs:label>Brettstein Cave</rdfs:label>
    </owl:NamedIndividual>
    


    <!-- http://purl.obolibrary.org/obo/GAZ_00015664 -->

    <owl:NamedIndividual rdf:about="http://purl.obolibrary.org/obo/GAZ_00015664">
        <obo:RO_0001025 rdf:resource="http://purl.obolibrary.org/obo/GAZ_00056798"/>
        <oboInOwl:hasOBONamespace>GAZ</oboInOwl:hasOBONamespace>
        <oboInOwl:id>GAZ:00015664</oboInOwl:id>
        <rdfs:label>Brieglersberg Cave</rdfs:label>
    </owl:NamedIndividual>
    


    <!-- http://purl.obolibrary.org/obo/GAZ_00015665 -->

    <owl:NamedIndividual rdf:about="http://purl.obolibrary.org/obo/GAZ_00015665">
        <obo:RO_0001025 rdf:resource="http://purl.obolibrary.org/obo/GAZ_00056798"/>
        <oboInOwl:hasOBONamespace>GAZ</oboInOwl:hasOBONamespace>
        <oboInOwl:id>GAZ:00015665</oboInOwl:id>
        <rdfs:label>Gamssulzen Cave</rdfs:label>
    </owl:NamedIndividual>
    


    <!-- http://purl.obolibrary.org/obo/GAZ_00015666 -->

    <owl:NamedIndividual rdf:about="http://purl.obolibrary.org/obo/GAZ_00015666">
        <obo:RO_0001025 rdf:resource="http://purl.obolibrary.org/obo/GAZ_00088601"/>
        <oboInOwl:hasOBONamespace>GAZ</oboInOwl:hasOBONamespace>
        <oboInOwl:id>GAZ:00015666</oboInOwl:id>
        <rdfs:label>Hartelsgraben Cave</rdfs:label>
    </owl:NamedIndividual>
    


    <!-- http://purl.obolibrary.org/obo/GAZ_00015678 -->

    <owl:NamedIndividual rdf:about="http://purl.obolibrary.org/obo/GAZ_00015678">
        <obo:RO_0001025 rdf:resource="http://purl.obolibrary.org/obo/GAZ_00056798"/>
        <obo:IAO_0000115>Eine Hohle im Toten Gebirge in Oberosterreich.</obo:IAO_0000115>
        <oboInOwl:hasOBONamespace>GAZ</oboInOwl:hasOBONamespace>
        <oboInOwl:id>GAZ:00015678</oboInOwl:id>
        <rdfs:label>Ramesch Cave</rdfs:label>
    </owl:NamedIndividual>
    


    <!-- http://purl.obolibrary.org/obo/GAZ_00015679 -->

    <owl:NamedIndividual rdf:about="http://purl.obolibrary.org/obo/GAZ_00015679">
        <obo:RO_0001025 rdf:resource="http://purl.obolibrary.org/obo/GAZ_00056798"/>
        <obo:IAO_0000115>A cave in Styria, Austria. It is located in the municipality of Bad Aussee at an altitude of approximately 2000 m.</obo:IAO_0000115>
        <oboInOwl:hasOBONamespace>GAZ</oboInOwl:hasOBONamespace>
        <oboInOwl:id>GAZ:00015679</oboInOwl:id>
        <rdfs:label>Salzofen Cave</rdfs:label>
    </owl:NamedIndividual>
    


    <!-- http://purl.obolibrary.org/obo/GAZ_00015680 -->

    <owl:NamedIndividual rdf:about="http://purl.obolibrary.org/obo/GAZ_00015680">
        <obo:RO_0001025 rdf:resource="http://purl.obolibrary.org/obo/GAZ_00103617"/>
        <oboInOwl:hasOBONamespace>GAZ</oboInOwl:hasOBONamespace>
        <oboInOwl:id>GAZ:00015680</oboInOwl:id>
        <rdfs:label>Schreiberwand Cave</rdfs:label>
    </owl:NamedIndividual>
    


    <!-- http://purl.obolibrary.org/obo/GAZ_00021159 -->

    <owl:NamedIndividual rdf:about="http://purl.obolibrary.org/obo/GAZ_00021159">
        <rdf:type rdf:resource="http://purl.obolibrary.org/obo/ENVO_00000856"/>
        <obo:RO_0001025 rdf:resource="http://purl.obolibrary.org/obo/GAZ_00144397"/>
        <obo:IAO_0000115>A municipality.</obo:IAO_0000115>
        <oboInOwl:hasOBONamespace>GAZ</oboInOwl:hasOBONamespace>
        <oboInOwl:id>GAZ:00021159</oboInOwl:id>
        <rdfs:label>Municipality of Culemborg</rdfs:label>
    </owl:NamedIndividual>
    


    <!-- http://purl.obolibrary.org/obo/GAZ_00021165 -->

    <owl:NamedIndividual rdf:about="http://purl.obolibrary.org/obo/GAZ_00021165">
        <rdf:type rdf:resource="http://purl.obolibrary.org/obo/ENVO_00000856"/>
        <obo:RO_0001025 rdf:resource="http://purl.obolibrary.org/obo/GAZ_00144397"/>
        <obo:IAO_0000115>A municipality.</obo:IAO_0000115>
        <oboInOwl:hasOBONamespace>GAZ</oboInOwl:hasOBONamespace>
        <oboInOwl:id>GAZ:00021165</oboInOwl:id>
        <rdfs:label>Municipality of Geldermalsen</rdfs:label>
    </owl:NamedIndividual>
    


    <!-- http://purl.obolibrary.org/obo/GAZ_00021176 -->

    <owl:NamedIndividual rdf:about="http://purl.obolibrary.org/obo/GAZ_00021176">
        <rdf:type rdf:resource="http://purl.obolibrary.org/obo/ENVO_00000856"/>
        <obo:RO_0001025 rdf:resource="http://purl.obolibrary.org/obo/GAZ_00144397"/>
        <obo:IAO_0000115>A municipality.</obo:IAO_0000115>
        <oboInOwl:hasOBONamespace>GAZ</oboInOwl:hasOBONamespace>
        <oboInOwl:id>GAZ:00021176</oboInOwl:id>
        <rdfs:label>Municipality of Tiel</rdfs:label>
    </owl:NamedIndividual>
    


    <!-- http://purl.obolibrary.org/obo/GAZ_00021216 -->

    <owl:NamedIndividual rdf:about="http://purl.obolibrary.org/obo/GAZ_00021216">
        <rdf:type rdf:resource="http://purl.obolibrary.org/obo/ENVO_00000856"/>
        <obo:RO_0001025 rdf:resource="http://purl.obolibrary.org/obo/GAZ_00144362"/>
        <obo:IAO_0000115>A municipality.</obo:IAO_0000115>
        <oboInOwl:hasOBONamespace>GAZ</oboInOwl:hasOBONamespace>
        <oboInOwl:id>GAZ:00021216</oboInOwl:id>
        <rdfs:label>Municipality of Kapelle</rdfs:label>
    </owl:NamedIndividual>
    


    <!-- http://purl.obolibrary.org/obo/GAZ_00021219 -->

    <owl:NamedIndividual rdf:about="http://purl.obolibrary.org/obo/GAZ_00021219">
        <rdf:type rdf:resource="http://purl.obolibrary.org/obo/ENVO_00000856"/>
        <obo:RO_0001025 rdf:resource="http://purl.obolibrary.org/obo/GAZ_00144371"/>
        <obo:IAO_0000115>A former municipality. Merged 1970.</obo:IAO_0000115>
        <oboInOwl:hasOBONamespace>GAZ</oboInOwl:hasOBONamespace>
        <oboInOwl:id>GAZ:00021219</oboInOwl:id>
        <rdfs:label>[Former] Municipality of Zuidzande</rdfs:label>
    </owl:NamedIndividual>
    


    <!-- http://purl.obolibrary.org/obo/GAZ_00021220 -->

    <owl:NamedIndividual rdf:about="http://purl.obolibrary.org/obo/GAZ_00021220">
        <rdf:type rdf:resource="http://purl.obolibrary.org/obo/ENVO_00000856"/>
        <obo:RO_0001025 rdf:resource="http://purl.obolibrary.org/obo/GAZ_00144371"/>
        <obo:IAO_0000115>A municipality.</obo:IAO_0000115>
        <oboInOwl:hasOBONamespace>GAZ</oboInOwl:hasOBONamespace>
        <oboInOwl:id>GAZ:00021220</oboInOwl:id>
        <rdfs:label>Municipality of Middelburg</rdfs:label>
    </owl:NamedIndividual>
    


    <!-- http://purl.obolibrary.org/obo/GAZ_00021221 -->

    <owl:NamedIndividual rdf:about="http://purl.obolibrary.org/obo/GAZ_00021221">
        <rdf:type rdf:resource="http://purl.obolibrary.org/obo/ENVO_00000856"/>
        <obo:RO_0001025 rdf:resource="http://purl.obolibrary.org/obo/GAZ_00144362"/>
        <obo:IAO_0000115>A municipality.</obo:IAO_0000115>
        <oboInOwl:hasOBONamespace>GAZ</oboInOwl:hasOBONamespace>
        <oboInOwl:id>GAZ:00021221</oboInOwl:id>
        <rdfs:label>Municipality of Reimerswaal</rdfs:label>
    </owl:NamedIndividual>
    


    <!-- http://purl.obolibrary.org/obo/GAZ_00021222 -->

    <owl:NamedIndividual rdf:about="http://purl.obolibrary.org/obo/GAZ_00021222">
        <rdf:type rdf:resource="http://purl.obolibrary.org/obo/ENVO_00000856"/>
        <obo:RO_0001025 rdf:resource="http://purl.obolibrary.org/obo/GAZ_00144373"/>
        <obo:IAO_0000115>A municipality.</obo:IAO_0000115>
        <oboInOwl:hasOBONamespace>GAZ</oboInOwl:hasOBONamespace>
        <oboInOwl:id>GAZ:00021222</oboInOwl:id>
        <rdfs:label>Municipality of Noord-Beveland</rdfs:label>
    </owl:NamedIndividual>
    


    <!-- http://purl.obolibrary.org/obo/GAZ_00021224 -->

    <owl:NamedIndividual rdf:about="http://purl.obolibrary.org/obo/GAZ_00021224">
        <rdf:type rdf:resource="http://purl.obolibrary.org/obo/ENVO_00000856"/>
        <obo:RO_0001025 rdf:resource="http://purl.obolibrary.org/obo/GAZ_00144362"/>
        <obo:IAO_0000115>A municipality.</obo:IAO_0000115>
        <oboInOwl:hasOBONamespace>GAZ</oboInOwl:hasOBONamespace>
        <oboInOwl:id>GAZ:00021224</oboInOwl:id>
        <rdfs:label>Municipality of Borsele</rdfs:label>
    </owl:NamedIndividual>
    


    <!-- http://purl.obolibrary.org/obo/GAZ_00021225 -->

    <owl:NamedIndividual rdf:about="http://purl.obolibrary.org/obo/GAZ_00021225">
        <obo:RO_0001025 rdf:resource="http://purl.obolibrary.org/obo/GAZ_00144371"/>
        <obo:IAO_0000115>A municipality in the southwestern Netherlands on the former island of Walcheren.</obo:IAO_0000115>
        <oboInOwl:hasOBONamespace>GAZ</oboInOwl:hasOBONamespace>
        <oboInOwl:id>GAZ:00021225</oboInOwl:id>
        <rdfs:label>Municipality of Vlissingen</rdfs:label>
    </owl:NamedIndividual>
    


    <!-- http://purl.obolibrary.org/obo/GAZ_00021226 -->

    <owl:NamedIndividual rdf:about="http://purl.obolibrary.org/obo/GAZ_00021226">
        <rdf:type rdf:resource="http://purl.obolibrary.org/obo/ENVO_00000856"/>
        <obo:RO_0001025 rdf:resource="http://purl.obolibrary.org/obo/GAZ_00090210"/>
        <obo:IAO_0000115>A municipality.</obo:IAO_0000115>
        <oboInOwl:hasOBONamespace>GAZ</oboInOwl:hasOBONamespace>
        <oboInOwl:id>GAZ:00021226</oboInOwl:id>
        <rdfs:label>Municipality of Tholen</rdfs:label>
    </owl:NamedIndividual>
    


    <!-- http://purl.obolibrary.org/obo/GAZ_00021228 -->

    <owl:NamedIndividual rdf:about="http://purl.obolibrary.org/obo/GAZ_00021228">
        <obo:RO_0001025 rdf:resource="http://purl.obolibrary.org/obo/GAZ_00144361"/>
        <obo:IAO_0000115>An island.</obo:IAO_0000115>
        <oboInOwl:hasOBONamespace>GAZ</oboInOwl:hasOBONamespace>
        <oboInOwl:id>GAZ:00021228</oboInOwl:id>
        <rdfs:label>Kadzand</rdfs:label>
    </owl:NamedIndividual>
    


    <!-- http://purl.obolibrary.org/obo/GAZ_00021229 -->

    <owl:NamedIndividual rdf:about="http://purl.obolibrary.org/obo/GAZ_00021229">
        <rdf:type rdf:resource="http://purl.obolibrary.org/obo/ENVO_00000856"/>
        <obo:RO_0001025 rdf:resource="http://purl.obolibrary.org/obo/GAZ_00043996"/>
        <obo:IAO_0000115>A municipality.</obo:IAO_0000115>
        <oboInOwl:hasOBONamespace>GAZ</oboInOwl:hasOBONamespace>
        <oboInOwl:id>GAZ:00021229</oboInOwl:id>
        <rdfs:label>Municipality of Schouwen-Duiveland</rdfs:label>
    </owl:NamedIndividual>
    


    <!-- http://purl.obolibrary.org/obo/GAZ_00021257 -->

    <owl:NamedIndividual rdf:about="http://purl.obolibrary.org/obo/GAZ_00021257">
        <rdf:type rdf:resource="http://purl.obolibrary.org/obo/ENVO_00000856"/>
        <obo:RO_0001025 rdf:resource="http://purl.obolibrary.org/obo/GAZ_00144381"/>
        <obo:IAO_0000115>A municipality.</obo:IAO_0000115>
        <oboInOwl:hasOBONamespace>GAZ</oboInOwl:hasOBONamespace>
        <oboInOwl:id>GAZ:00021257</oboInOwl:id>
        <rdfs:label>Municipality of Binnenmaas</rdfs:label>
    </owl:NamedIndividual>
    


    <!-- http://purl.obolibrary.org/obo/GAZ_00021258 -->

    <owl:NamedIndividual rdf:about="http://purl.obolibrary.org/obo/GAZ_00021258">
        <rdf:type rdf:resource="http://purl.obolibrary.org/obo/ENVO_00000856"/>
        <obo:RO_0001025 rdf:resource="http://purl.obolibrary.org/obo/GAZ_00144381"/>
        <obo:IAO_0000115>A municipality.</obo:IAO_0000115>
        <oboInOwl:hasOBONamespace>GAZ</oboInOwl:hasOBONamespace>
        <oboInOwl:id>GAZ:00021258</oboInOwl:id>
        <rdfs:label>Municipality of Cromstrijen</rdfs:label>
    </owl:NamedIndividual>
    


    <!-- http://purl.obolibrary.org/obo/GAZ_00021260 -->

    <owl:NamedIndividual rdf:about="http://purl.obolibrary.org/obo/GAZ_00021260">
        <rdf:type rdf:resource="http://purl.obolibrary.org/obo/ENVO_00000856"/>
        <obo:RO_0001025 rdf:resource="http://purl.obolibrary.org/obo/GAZ_00043990"/>
        <obo:IAO_0000115>A municipality.</obo:IAO_0000115>
        <oboInOwl:hasOBONamespace>GAZ</oboInOwl:hasOBONamespace>
        <oboInOwl:id>GAZ:00021260</oboInOwl:id>
        <rdfs:label>Municipality of Barendrecht</rdfs:label>
    </owl:NamedIndividual>
    


    <!-- http://purl.obolibrary.org/obo/GAZ_00021269 -->

    <owl:NamedIndividual rdf:about="http://purl.obolibrary.org/obo/GAZ_00021269">
        <rdf:type rdf:resource="http://purl.obolibrary.org/obo/ENVO_00000856"/>
        <obo:RO_0001025 rdf:resource="http://purl.obolibrary.org/obo/GAZ_00043988"/>
        <obo:IAO_0000115>A municipality.</obo:IAO_0000115>
        <oboInOwl:hasOBONamespace>GAZ</oboInOwl:hasOBONamespace>
        <oboInOwl:id>GAZ:00021269</oboInOwl:id>
        <rdfs:label>Municipality of Dirksland</rdfs:label>
    </owl:NamedIndividual>
    


    <!-- http://purl.obolibrary.org/obo/GAZ_00021272 -->

    <owl:NamedIndividual rdf:about="http://purl.obolibrary.org/obo/GAZ_00021272">
        <rdf:type rdf:resource="http://purl.obolibrary.org/obo/ENVO_00000856"/>
        <obo:RO_0001025 rdf:resource="http://purl.obolibrary.org/obo/GAZ_00043988"/>
        <obo:IAO_0000115>A municipality.</obo:IAO_0000115>
        <oboInOwl:hasOBONamespace>GAZ</oboInOwl:hasOBONamespace>
        <oboInOwl:id>GAZ:00021272</oboInOwl:id>
        <rdfs:label>Municipality of Goedereede</rdfs:label>
    </owl:NamedIndividual>
    


    <!-- http://purl.obolibrary.org/obo/GAZ_00021273 -->

    <owl:NamedIndividual rdf:about="http://purl.obolibrary.org/obo/GAZ_00021273">
        <rdf:type rdf:resource="http://purl.obolibrary.org/obo/ENVO_00000856"/>
        <obo:RO_0001025 rdf:resource="http://purl.obolibrary.org/obo/GAZ_00144381"/>
        <obo:IAO_0000115>A municipality.</obo:IAO_0000115>
        <oboInOwl:hasOBONamespace>GAZ</oboInOwl:hasOBONamespace>
        <oboInOwl:id>GAZ:00021273</oboInOwl:id>
        <rdfs:label>Municipality of Korendijk</rdfs:label>
    </owl:NamedIndividual>
    


    <!-- http://purl.obolibrary.org/obo/GAZ_00021285 -->

    <owl:NamedIndividual rdf:about="http://purl.obolibrary.org/obo/GAZ_00021285">
        <rdf:type rdf:resource="http://purl.obolibrary.org/obo/ENVO_00000856"/>
        <obo:RO_0001025 rdf:resource="http://purl.obolibrary.org/obo/GAZ_00043990"/>
        <obo:IAO_0000115>A municipality.</obo:IAO_0000115>
        <oboInOwl:hasOBONamespace>GAZ</oboInOwl:hasOBONamespace>
        <oboInOwl:id>GAZ:00021285</oboInOwl:id>
        <rdfs:label>Municipality of Hendrik-Ido-Ambacht</rdfs:label>
    </owl:NamedIndividual>
    


    <!-- http://purl.obolibrary.org/obo/GAZ_00021287 -->

    <owl:NamedIndividual rdf:about="http://purl.obolibrary.org/obo/GAZ_00021287">
        <rdf:type rdf:resource="http://purl.obolibrary.org/obo/ENVO_00000856"/>
        <obo:RO_0001025 rdf:resource="http://purl.obolibrary.org/obo/GAZ_00144381"/>
        <obo:IAO_0000115>A municipality.</obo:IAO_0000115>
        <oboInOwl:hasOBONamespace>GAZ</oboInOwl:hasOBONamespace>
        <oboInOwl:id>GAZ:00021287</oboInOwl:id>
        <rdfs:label>Municipality of Oud-Beijerland</rdfs:label>
    </owl:NamedIndividual>
    


    <!-- http://purl.obolibrary.org/obo/GAZ_00021293 -->

    <owl:NamedIndividual rdf:about="http://purl.obolibrary.org/obo/GAZ_00021293">
        <rdf:type rdf:resource="http://purl.obolibrary.org/obo/ENVO_00000856"/>
        <obo:RO_0001025 rdf:resource="http://purl.obolibrary.org/obo/GAZ_00043988"/>
        <obo:IAO_0000115>A municipality.</obo:IAO_0000115>
        <oboInOwl:hasOBONamespace>GAZ</oboInOwl:hasOBONamespace>
        <oboInOwl:id>GAZ:00021293</oboInOwl:id>
        <rdfs:label>Municipality of Oostflakkee</rdfs:label>
    </owl:NamedIndividual>
    


    <!-- http://purl.obolibrary.org/obo/GAZ_00021304 -->

    <owl:NamedIndividual rdf:about="http://purl.obolibrary.org/obo/GAZ_00021304">
        <rdf:type rdf:resource="http://purl.obolibrary.org/obo/ENVO_00000856"/>
        <obo:RO_0001025 rdf:resource="http://purl.obolibrary.org/obo/GAZ_00043988"/>
        <obo:IAO_0000115>A municipality.</obo:IAO_0000115>
        <oboInOwl:hasOBONamespace>GAZ</oboInOwl:hasOBONamespace>
        <oboInOwl:id>GAZ:00021304</oboInOwl:id>
        <rdfs:label>Municipality of Middelharnis</rdfs:label>
    </owl:NamedIndividual>
    


    <!-- http://purl.obolibrary.org/obo/GAZ_00021312 -->

    <owl:NamedIndividual rdf:about="http://purl.obolibrary.org/obo/GAZ_00021312">
        <rdf:type rdf:resource="http://purl.obolibrary.org/obo/ENVO_00000856"/>
        <obo:RO_0001025 rdf:resource="http://purl.obolibrary.org/obo/GAZ_00144381"/>
        <obo:IAO_0000115>A municipality.</obo:IAO_0000115>
        <oboInOwl:hasOBONamespace>GAZ</oboInOwl:hasOBONamespace>
        <oboInOwl:id>GAZ:00021312</oboInOwl:id>
        <rdfs:label>Municipality of Strijen</rdfs:label>
    </owl:NamedIndividual>
    


    <!-- http://purl.obolibrary.org/obo/GAZ_00021319 -->

    <owl:NamedIndividual rdf:about="http://purl.obolibrary.org/obo/GAZ_00021319">
        <rdf:type rdf:resource="http://purl.obolibrary.org/obo/ENVO_00000856"/>
        <obo:RO_0001025 rdf:resource="http://purl.obolibrary.org/obo/GAZ_00043990"/>
        <obo:IAO_0000115>A municipality.</obo:IAO_0000115>
        <oboInOwl:hasOBONamespace>GAZ</oboInOwl:hasOBONamespace>
        <oboInOwl:id>GAZ:00021319</oboInOwl:id>
        <rdfs:label>Municipality of Ridderkerk</rdfs:label>
    </owl:NamedIndividual>
    


    <!-- http://purl.obolibrary.org/obo/GAZ_00043216 -->

    <owl:NamedIndividual rdf:about="http://purl.obolibrary.org/obo/GAZ_00043216">
        <obo:RO_0001025 rdf:resource="http://purl.obolibrary.org/obo/GAZ_00008111"/>
        <obo:IAO_0000115>A land-tied lacustrine island. A World Heritage Site.</obo:IAO_0000115>
        <oboInOwl:hasOBONamespace>GAZ</oboInOwl:hasOBONamespace>
        <oboInOwl:id>GAZ:00043216</oboInOwl:id>
        <rdfs:label>Reichenau</rdfs:label>
    </owl:NamedIndividual>
    


    <!-- http://purl.obolibrary.org/obo/GAZ_00043981 -->

    <owl:NamedIndividual rdf:about="http://purl.obolibrary.org/obo/GAZ_00043981">
        <obo:RO_0001025 rdf:resource="http://purl.obolibrary.org/obo/GAZ_00008262"/>
        <obo:IAO_0000115>An island near Bad Honnef in the Rhine, administratively part of Remagen in Rhineland-Palatinate.</obo:IAO_0000115>
        <oboInOwl:hasOBONamespace>GAZ</oboInOwl:hasOBONamespace>
        <oboInOwl:id>GAZ:00043981</oboInOwl:id>
        <rdfs:label>Nonnenwerth</rdfs:label>
    </owl:NamedIndividual>
    


    <!-- http://purl.obolibrary.org/obo/GAZ_00043988 -->

    <owl:NamedIndividual rdf:about="http://purl.obolibrary.org/obo/GAZ_00043988">
        <obo:RO_0001025 rdf:resource="http://purl.obolibrary.org/obo/GAZ_00144376"/>
        <obo:IAO_0000115>The southernmost delta island of the province of South Holland, Netherlands. It is separated from Voorne-Putten and Hoeksche Waard by the Haringvliet, from the mainland of North Brabant by the Volkerak, and from Schouwen-Duiveland by Lake Grevelingen.</obo:IAO_0000115>
        <oboInOwl:hasOBONamespace>GAZ</oboInOwl:hasOBONamespace>
        <oboInOwl:id>GAZ:00043988</oboInOwl:id>
        <rdfs:label>Goeree-Overflakkee</rdfs:label>
    </owl:NamedIndividual>
    


    <!-- http://purl.obolibrary.org/obo/GAZ_00043990 -->

    <owl:NamedIndividual rdf:about="http://purl.obolibrary.org/obo/GAZ_00043990">
        <rdf:type rdf:resource="http://purl.obolibrary.org/obo/ENVO_00000423"/>
        <obo:RO_0001025 rdf:resource="http://purl.obolibrary.org/obo/GAZ_00144376"/>
        <obo:IAO_0000115>A fluvial island between the Nieuwe Maas, Noord and Oude Maas branches rivers of the Rhine-Meuse delta in the Dutch province of Zuid Holland. The city of Rotterdam now occupies most of the northern part of the island.</obo:IAO_0000115>
        <oboInOwl:hasOBONamespace>GAZ</oboInOwl:hasOBONamespace>
        <oboInOwl:id>GAZ:00043990</oboInOwl:id>
        <rdfs:label>IJsselmonde</rdfs:label>
    </owl:NamedIndividual>
    


    <!-- http://purl.obolibrary.org/obo/GAZ_00043994 -->

    <owl:NamedIndividual rdf:about="http://purl.obolibrary.org/obo/GAZ_00043994">
        <obo:RO_0001025 rdf:resource="http://purl.obolibrary.org/obo/GAZ_00144376"/>
        <obo:IAO_0000115>An island bordered by the rivers Oude Maas, Beneden Merwede, Nieuwe Merwede, Hollands Diep, and Dordtsche Kil. Occupied by the Municipality of Dordrecht.</obo:IAO_0000115>
        <oboInOwl:hasOBONamespace>GAZ</oboInOwl:hasOBONamespace>
        <oboInOwl:id>GAZ:00043994</oboInOwl:id>
        <rdfs:label>Eiland van Dordrecht</rdfs:label>
    </owl:NamedIndividual>
    


    <!-- http://purl.obolibrary.org/obo/GAZ_00043995 -->

    <owl:NamedIndividual rdf:about="http://purl.obolibrary.org/obo/GAZ_00043995">
        <obo:RO_0001025 rdf:resource="http://purl.obolibrary.org/obo/GAZ_00021273"/>
        <obo:IAO_0000115>An island in the Dutch province of South Holland. It is a part of the municipality of Korendijk, and lies about 11 km south of Spijkenisse.</obo:IAO_0000115>
        <oboInOwl:hasOBONamespace>GAZ</oboInOwl:hasOBONamespace>
        <oboInOwl:id>GAZ:00043995</oboInOwl:id>
        <rdfs:label>Tiengemeten</rdfs:label>
    </owl:NamedIndividual>
    


    <!-- http://purl.obolibrary.org/obo/GAZ_00043996 -->

    <owl:NamedIndividual rdf:about="http://purl.obolibrary.org/obo/GAZ_00043996">
        <obo:RO_0001025 rdf:resource="http://purl.obolibrary.org/obo/GAZ_00090210"/>
        <obo:IAO_0000115>An island in the southwestern Netherlands. The Brouwersdam goes from Schouwen-Duiveland to Goedereede, the west part of the island of Goeree-Overflakkee in South Holland.</obo:IAO_0000115>
        <oboInOwl:hasOBONamespace>GAZ</oboInOwl:hasOBONamespace>
        <oboInOwl:id>GAZ:00043996</oboInOwl:id>
        <rdfs:label>Schouwen-Duiveland</rdfs:label>
    </owl:NamedIndividual>
    


    <!-- http://purl.obolibrary.org/obo/GAZ_00043997 -->

    <owl:NamedIndividual rdf:about="http://purl.obolibrary.org/obo/GAZ_00043997">
        <obo:RO_0001025 rdf:resource="http://purl.obolibrary.org/obo/GAZ_00021226"/>
        <obo:IAO_0000115>A former island, now a peninsula.</obo:IAO_0000115>
        <oboInOwl:hasOBONamespace>GAZ</oboInOwl:hasOBONamespace>
        <oboInOwl:id>GAZ:00043997</oboInOwl:id>
        <rdfs:label>Sint Philipsland</rdfs:label>
    </owl:NamedIndividual>
    


    <!-- http://purl.obolibrary.org/obo/GAZ_00043998 -->

    <owl:NamedIndividual rdf:about="http://purl.obolibrary.org/obo/GAZ_00043998">
        <obo:RO_0001025 rdf:resource="http://purl.obolibrary.org/obo/GAZ_00021226"/>
        <obo:IAO_0000115>A former island, now a peninsula.</obo:IAO_0000115>
        <oboInOwl:hasOBONamespace>GAZ</oboInOwl:hasOBONamespace>
        <oboInOwl:id>GAZ:00043998</oboInOwl:id>
        <rdfs:label>Tholen [Island]</rdfs:label>
    </owl:NamedIndividual>
    


    <!-- http://purl.obolibrary.org/obo/GAZ_00044655 -->

    <owl:NamedIndividual rdf:about="http://purl.obolibrary.org/obo/GAZ_00044655">
        <rdf:type rdf:resource="http://purl.obolibrary.org/obo/ENVO_00000423"/>
        <obo:IAO_0000115>A fluvial island.</obo:IAO_0000115>
        <oboInOwl:hasOBONamespace>GAZ</oboInOwl:hasOBONamespace>
        <oboInOwl:id>GAZ:00044655</oboInOwl:id>
        <rdfs:label>Insel Grien</rdfs:label>
    </owl:NamedIndividual>
    


    <!-- http://purl.obolibrary.org/obo/GAZ_00044657 -->

    <owl:NamedIndividual rdf:about="http://purl.obolibrary.org/obo/GAZ_00044657">
        <obo:RO_0001025 rdf:resource="http://purl.obolibrary.org/obo/GAZ_00008262"/>
        <oboInOwl:hasOBONamespace>GAZ</oboInOwl:hasOBONamespace>
        <oboInOwl:id>GAZ:00044657</oboInOwl:id>
        <rdfs:label>Insel Rheinau</rdfs:label>
    </owl:NamedIndividual>
    


    <!-- http://purl.obolibrary.org/obo/GAZ_00044659 -->

    <owl:NamedIndividual rdf:about="http://purl.obolibrary.org/obo/GAZ_00044659">
        <obo:RO_0001025 rdf:resource="http://purl.obolibrary.org/obo/GAZ_00008262"/>
        <obo:IAO_0000115>Die Hauptinsel einer kleinen Inselgruppe im Rhein beziehungsweise im Untersee des Bodensees zwischen Stein am Rhein und Eschenz.</obo:IAO_0000115>
        <oboInOwl:hasOBONamespace>GAZ</oboInOwl:hasOBONamespace>
        <oboInOwl:id>GAZ:00044659</oboInOwl:id>
        <rdfs:label>Insel Werd</rdfs:label>
    </owl:NamedIndividual>
    


    <!-- http://purl.obolibrary.org/obo/GAZ_00044675 -->

    <owl:NamedIndividual rdf:about="http://purl.obolibrary.org/obo/GAZ_00044675">
        <obo:IAO_0000115>A reservoir in the Canton of Fribourg, Switzerland. It was formed between the cities of Bulle and Fribourg, by building the Rossens Dam. Constructed 1948.</obo:IAO_0000115>
        <oboInOwl:hasOBONamespace>GAZ</oboInOwl:hasOBONamespace>
        <oboInOwl:id>GAZ:00044675</oboInOwl:id>
        <rdfs:label>Lac de la Gruyere</rdfs:label>
    </owl:NamedIndividual>
    


    <!-- http://purl.obolibrary.org/obo/GAZ_00044676 -->

    <owl:NamedIndividual rdf:about="http://purl.obolibrary.org/obo/GAZ_00044676">
        <obo:RO_0001025 rdf:resource="http://purl.obolibrary.org/obo/GAZ_00044675"/>
        <obo:IAO_0000115>An island in Lac de la Gruyere.</obo:IAO_0000115>
        <oboInOwl:hasOBONamespace>GAZ</oboInOwl:hasOBONamespace>
        <oboInOwl:id>GAZ:00044676</oboInOwl:id>
        <rdfs:label>Ile d&apos;Ogoz</rdfs:label>
    </owl:NamedIndividual>
    


    <!-- http://purl.obolibrary.org/obo/GAZ_00051913 -->

    <owl:NamedIndividual rdf:about="http://purl.obolibrary.org/obo/GAZ_00051913">
        <obo:IAO_0000115>The eastern half of the Alps, usually defined as the area east of the Splugen Pass in eastern Switzerland. North of the Splugen Pass, the Posterior Rhine forms the border, and south of the pass, the Liro river and Lake Como form the boundary line. The Eastern Alps include parts of Switzerland, most of Austria and Liechtenstein, as well as parts of southern Germany, northern Italy and Slovenia. The eastern border is formed by the Wienerwald (Vienna Woods) and the Viennese basin, which is the transition zone to the Carpathian mountains.</obo:IAO_0000115>
        <oboInOwl:hasOBONamespace>GAZ</oboInOwl:hasOBONamespace>
        <oboInOwl:id>GAZ:00051913</oboInOwl:id>
        <rdfs:label>Eastern Alps</rdfs:label>
    </owl:NamedIndividual>
    


    <!-- http://purl.obolibrary.org/obo/GAZ_00051914 -->

    <owl:NamedIndividual rdf:about="http://purl.obolibrary.org/obo/GAZ_00051914">
        <obo:RO_0001025 rdf:resource="http://purl.obolibrary.org/obo/GAZ_00051913"/>
        <obo:IAO_0000115>The core ranges of the Eastern Alps with the highest peaks, located between the Northern Limestone Alps and the Southern Limestone Alps, from which they differ in geological composition. They extend from the Bernina Range in Graubunden to the west as far as to the lower promontories east of the Mura such as the Hochwechsel in Styria in the east.</obo:IAO_0000115>
        <oboInOwl:hasOBONamespace>GAZ</oboInOwl:hasOBONamespace>
        <oboInOwl:id>GAZ:00051914</oboInOwl:id>
        <rdfs:label>Central Eastern Alps</rdfs:label>
    </owl:NamedIndividual>
    


    <!-- http://purl.obolibrary.org/obo/GAZ_00051915 -->

    <owl:NamedIndividual rdf:about="http://purl.obolibrary.org/obo/GAZ_00051915">
        <obo:RO_0001025 rdf:resource="http://purl.obolibrary.org/obo/GAZ_00051913"/>
        <obo:IAO_0000115>The ranges of the Eastern Alps north of the Central Eastern Alps. The distinction from the latter group, where the higher peaks are located, is based on differences in geological composition. The Northern Limestone Alps extend from the Bregenzerwald in Vorarlberg in the west to the Wienerwald in Lower Austria and Vienna in the east.</obo:IAO_0000115>
        <oboInOwl:hasOBONamespace>GAZ</oboInOwl:hasOBONamespace>
        <oboInOwl:id>GAZ:00051915</oboInOwl:id>
        <rdfs:label>Northern Limestone Alps</rdfs:label>
    </owl:NamedIndividual>
    


    <!-- http://purl.obolibrary.org/obo/GAZ_00051916 -->

    <owl:NamedIndividual rdf:about="http://purl.obolibrary.org/obo/GAZ_00051916">
        <obo:RO_0001025 rdf:resource="http://purl.obolibrary.org/obo/GAZ_00051913"/>
        <obo:IAO_0000115>The ranges of the Eastern Alps south of the Central Eastern Alps. The distinction from the latter group, where the higher peaks are located, is based on differences in geological composition. The Southern Limestone Alps extend from the Sobretta-Gavia Alps in Lombardy in the west to the Pohorje in Slovenia in the east.</obo:IAO_0000115>
        <oboInOwl:hasOBONamespace>GAZ</oboInOwl:hasOBONamespace>
        <oboInOwl:id>GAZ:00051916</oboInOwl:id>
        <rdfs:label>Southern Limestone Alps</rdfs:label>
    </owl:NamedIndividual>
    


    <!-- http://purl.obolibrary.org/obo/GAZ_00051917 -->

    <owl:NamedIndividual rdf:about="http://purl.obolibrary.org/obo/GAZ_00051917">
        <oboInOwl:hasOBONamespace>GAZ</oboInOwl:hasOBONamespace>
        <oboInOwl:id>GAZ:00051917</oboInOwl:id>
        <rdfs:label>Western Alps</rdfs:label>
    </owl:NamedIndividual>
    


    <!-- http://purl.obolibrary.org/obo/GAZ_00056783 -->

    <owl:NamedIndividual rdf:about="http://purl.obolibrary.org/obo/GAZ_00056783">
        <obo:RO_0001025 rdf:resource="http://purl.obolibrary.org/obo/GAZ_00051914"/>
        <obo:IAO_0000115>A mountain range which forms part of the Central Eastern Alps. They are located in northern Lombardy and named after the city Bergamo, south of the mountains. The Bergamo Alps stretch between Lake Como and Lake Iseo. They are separated from the Bregaglia and Bernina ranges in the north by the Adda River valley (Valtellina); from the Ortler Alps in the north-east by the Aprica Pass; from the Adamello-Presanella group in the east by the Oglio valley (Val Camonica).</obo:IAO_0000115>
        <oboInOwl:hasOBONamespace>GAZ</oboInOwl:hasOBONamespace>
        <oboInOwl:id>GAZ:00056783</oboInOwl:id>
        <rdfs:label>Bergamo Alps</rdfs:label>
    </owl:NamedIndividual>
    


    <!-- http://purl.obolibrary.org/obo/GAZ_00056784 -->

    <owl:NamedIndividual rdf:about="http://purl.obolibrary.org/obo/GAZ_00056784">
        <obo:RO_0001025 rdf:resource="http://purl.obolibrary.org/obo/GAZ_00051914"/>
        <obo:IAO_0000115>The highest range of the Alps east of the Brenner Pass, includes the highest mountains in Austria. The range is part of the Central Eastern Alps. It is in the Austrian states of Salzburg, Carinthia, and East Tyrol - with a small part in the Italian South Tyrol. The range is bounded by the Salzach valley to the north (separating it from the Kitzbuhel Alps); the Mur valley and the Murtorl Pass to the east (separating it from the Niedere Tauern); the Drave valley to the south (separating it from the Southern Limestone Alps); and the Birnlucke pass to the west (separating it from the Zillertal Alps).</obo:IAO_0000115>
        <oboInOwl:hasOBONamespace>GAZ</oboInOwl:hasOBONamespace>
        <oboInOwl:id>GAZ:00056784</oboInOwl:id>
        <rdfs:label>Hohe Tauern</rdfs:label>
    </owl:NamedIndividual>
    


    <!-- http://purl.obolibrary.org/obo/GAZ_00056785 -->

    <owl:NamedIndividual rdf:about="http://purl.obolibrary.org/obo/GAZ_00056785">
        <obo:RO_0001025 rdf:resource="http://purl.obolibrary.org/obo/GAZ_00051914"/>
        <obo:IAO_0000115>A mountain range surrounding Kitzbuhel in Austria, spanning from the Zillertal in the west to the Saalachtal and Zell am See in the east. It is bordered on the South by the Gerlospass and the upper Salzachtal, on the North the Inntal (valley of the river Inn) up to Worgl, and to the East by the Solland, St. Johann in Tirol, Fieberbrunn, the Griessenpass and Leogang.</obo:IAO_0000115>
        <oboInOwl:hasOBONamespace>GAZ</oboInOwl:hasOBONamespace>
        <oboInOwl:id>GAZ:00056785</oboInOwl:id>
        <rdfs:label>Kitzbuhler Alps</rdfs:label>
    </owl:NamedIndividual>
    


    <!-- http://purl.obolibrary.org/obo/GAZ_00056786 -->

    <owl:NamedIndividual rdf:about="http://purl.obolibrary.org/obo/GAZ_00056786">
        <obo:RO_0001025 rdf:resource="http://purl.obolibrary.org/obo/GAZ_00051914"/>
        <obo:IAO_0000115>A mountain range in central Austria, part of the Central Eastern Alps. They lie on the main chain of the Alps, directly east of the Hohe Tauern, in parts of Salzburger Land and Styria, from Murtorl in the west to the Schoberpass in the east.</obo:IAO_0000115>
        <oboInOwl:hasOBONamespace>GAZ</oboInOwl:hasOBONamespace>
        <oboInOwl:id>GAZ:00056786</oboInOwl:id>
        <rdfs:label>Niedere Tauern</rdfs:label>
    </owl:NamedIndividual>
    


    <!-- http://purl.obolibrary.org/obo/GAZ_00056787 -->

    <owl:NamedIndividual rdf:about="http://purl.obolibrary.org/obo/GAZ_00056787">
        <obo:RO_0001025 rdf:resource="http://purl.obolibrary.org/obo/GAZ_00060622"/>
        <obo:IAO_0000115>A mountain range in the central Alps of Europe, part of the Central Eastern Alps. They are arrayed at the head of the Otztal, a side valley of the Inn River southwest of Innsbruck, Austria; the line of summits forms part of Austria&apos;s border with Italy. The western border is the Resia Pass, while on the east the range is separated from the Stubai Alps by the Timmelsjoch.</obo:IAO_0000115>
        <oboInOwl:hasOBONamespace>GAZ</oboInOwl:hasOBONamespace>
        <oboInOwl:id>GAZ:00056787</oboInOwl:id>
        <rdfs:label>Otztal Alps</rdfs:label>
    </owl:NamedIndividual>
    


    <!-- http://purl.obolibrary.org/obo/GAZ_00056788 -->

    <owl:NamedIndividual rdf:about="http://purl.obolibrary.org/obo/GAZ_00056788">
        <obo:RO_0001025 rdf:resource="http://purl.obolibrary.org/obo/GAZ_00051914"/>
        <obo:IAO_0000115>A mountain range that is a part of the Central Eastern Alps along the Italian/Swiss and Austrian/Swiss borders, mostly located in the Graubunden canton in eastern Switzerland. The Rhaetian Alps contain the Albula, Bernina, Bregaglia, Ratikon and Silvretta subranges. The Swiss National Park is located in the eastern segment.</obo:IAO_0000115>
        <oboInOwl:hasOBONamespace>GAZ</oboInOwl:hasOBONamespace>
        <oboInOwl:id>GAZ:00056788</oboInOwl:id>
        <rdfs:label>Rhaetian Alps</rdfs:label>
    </owl:NamedIndividual>
    


    <!-- http://purl.obolibrary.org/obo/GAZ_00056790 -->

    <owl:NamedIndividual rdf:about="http://purl.obolibrary.org/obo/GAZ_00056790">
        <obo:RO_0001025 rdf:resource="http://purl.obolibrary.org/obo/GAZ_00060622"/>
        <obo:IAO_0000115>A mountain range in the Central Eastern Alps of Europe. It is named after the Stubaital valley to its east. It is located southwest of Innsbruck, Austria, and several summits of the range form part of Austria&apos;s border with Italy. The range is bounded by the Inn River valley to the north; the Sill River valley (Wipptal) and the Brenner Pass to the east (separating it from the Zillertal Alps); the Otztal and Timmelsjoch to the west (separating it from the Otztal Alps), and to the south by tributaries of the Passirio River and Isarco River.</obo:IAO_0000115>
        <oboInOwl:hasOBONamespace>GAZ</oboInOwl:hasOBONamespace>
        <oboInOwl:id>GAZ:00056790</oboInOwl:id>
        <rdfs:label>Stubai Alps</rdfs:label>
    </owl:NamedIndividual>
    


    <!-- http://purl.obolibrary.org/obo/GAZ_00056791 -->

    <owl:NamedIndividual rdf:about="http://purl.obolibrary.org/obo/GAZ_00056791">
        <obo:RO_0001025 rdf:resource="http://purl.obolibrary.org/obo/GAZ_00051914"/>
        <obo:IAO_0000115>A small mountain range of the Alps in Austria. The range is named after the Tux Valley, a side valley of the Ziller Valley. It is part of the Central Eastern Alps. The range is bounded by the Inn valley to the north (separating it from the Karwendel); the lower Ziller valley to the east (separating it from the Kitzbuhel Alps); the Tuxerjoch pass and the Tux Valley to the south (separating it from the Zillertal Alps); the Wipptal to the west (separating it from the Stubai Alps).</obo:IAO_0000115>
        <oboInOwl:hasOBONamespace>GAZ</oboInOwl:hasOBONamespace>
        <oboInOwl:id>GAZ:00056791</oboInOwl:id>
        <rdfs:label>Tux Alps</rdfs:label>
    </owl:NamedIndividual>
    


    <!-- http://purl.obolibrary.org/obo/GAZ_00056792 -->

    <owl:NamedIndividual rdf:about="http://purl.obolibrary.org/obo/GAZ_00056792">
        <obo:RO_0001025 rdf:resource="http://purl.obolibrary.org/obo/GAZ_00051914"/>
        <obo:IAO_0000115>A mountain range of the Alps on the border of Austria and Italy. The range is named after the Zillertal (Ziller river valley), on its north. It is part of the Central Eastern Alps. The range is bounded by the Tuxerjoch pass to the north (separating it from the Tux Alps); the Birnlucke-Forcella del Picco Pass to the east (separating it from the Hohe Tauern); the Isarco River and its tributary Rienz-Rienza to the south (separating it from the Southern Limestone Alps); the Brenner Pass to the west (separating it from the Stubai Alps).</obo:IAO_0000115>
        <oboInOwl:hasOBONamespace>GAZ</oboInOwl:hasOBONamespace>
        <oboInOwl:id>GAZ:00056792</oboInOwl:id>
        <rdfs:label>Zillertal Alps</rdfs:label>
    </owl:NamedIndividual>
    


    <!-- http://purl.obolibrary.org/obo/GAZ_00056793 -->

    <owl:NamedIndividual rdf:about="http://purl.obolibrary.org/obo/GAZ_00056793">
        <obo:RO_0001025 rdf:resource="http://purl.obolibrary.org/obo/GAZ_00051914"/>
        <obo:IAO_0000115>A mountain range of the Central Eastern Alps at the border of Tirol and Vorarlberg.</obo:IAO_0000115>
        <oboInOwl:hasOBONamespace>GAZ</oboInOwl:hasOBONamespace>
        <oboInOwl:id>GAZ:00056793</oboInOwl:id>
        <rdfs:label>Verwall Alps</rdfs:label>
    </owl:NamedIndividual>
    


    <!-- http://purl.obolibrary.org/obo/GAZ_00056794 -->

    <owl:NamedIndividual rdf:about="http://purl.obolibrary.org/obo/GAZ_00056794">
        <rdf:type rdf:resource="http://purl.obolibrary.org/obo/ENVO_00000106"/>
        <obo:RO_0001025 rdf:resource="http://purl.obolibrary.org/obo/GAZ_00051916"/>
        <obo:IAO_0000115>A range of the Southern Limestone Alps at the borders of East Tyrol, Carinthia and Friuli, between Austria and Italy. They extend from east to west for about 100 km between the Drava, Gail and Tagliamento.</obo:IAO_0000115>
        <oboInOwl:hasOBONamespace>GAZ</oboInOwl:hasOBONamespace>
        <oboInOwl:id>GAZ:00056794</oboInOwl:id>
        <rdfs:label>Carnic Alps</rdfs:label>
    </owl:NamedIndividual>
    


    <!-- http://purl.obolibrary.org/obo/GAZ_00056795 -->

    <owl:NamedIndividual rdf:about="http://purl.obolibrary.org/obo/GAZ_00056795">
        <obo:RO_0001025 rdf:resource="http://purl.obolibrary.org/obo/GAZ_00051916"/>
        <obo:IAO_0000115>A mountain range in the Italian Alps. It is part of the Southern Limestone Alps. It is located in the province of Trento. The Brenta Group is separated from the Ortler Alps in the north by the Noce valley; from the Adamello-Presanella group in the west by the Campo Carlo Magno Pass and the river Sarca; from the Fiemme Alps in the east by the Adige valley.</obo:IAO_0000115>
        <oboInOwl:hasOBONamespace>GAZ</oboInOwl:hasOBONamespace>
        <oboInOwl:id>GAZ:00056795</oboInOwl:id>
        <rdfs:label>Brenta Group</rdfs:label>
    </owl:NamedIndividual>
    


    <!-- http://purl.obolibrary.org/obo/GAZ_00056796 -->

    <owl:NamedIndividual rdf:about="http://purl.obolibrary.org/obo/GAZ_00056796">
        <obo:RO_0001025 rdf:resource="http://purl.obolibrary.org/obo/GAZ_00051915"/>
        <obo:IAO_0000115>Un massif des Prealpes orientales septentrionales. Il s&apos;eleve entre l&apos;Autriche (Land de Salzbourg) et l&apos;Allemagne (Baviere). Leur nom provient de la ville de Berchtesgaden, au sein du massif. Le massif est entoure par le massif du Salzkammergut au nord-est, le massif de Tennen a l&apos;est, le Hohe Tauern au sud, les Alpes de Kitzbuhel au sud-ouest, les massifs de Lofer et Leogang a l&apos;ouest et les Alpes de Chiemgau au nord-ouest. Il est borde a l&apos;est par la Salzach et baigne par le Konigssee et le Zeller See.</obo:IAO_0000115>
        <oboInOwl:hasOBONamespace>GAZ</oboInOwl:hasOBONamespace>
        <oboInOwl:id>GAZ:00056796</oboInOwl:id>
        <rdfs:label>Berchtesgaden Alps</rdfs:label>
    </owl:NamedIndividual>
    


    <!-- http://purl.obolibrary.org/obo/GAZ_00056797 -->

    <owl:NamedIndividual rdf:about="http://purl.obolibrary.org/obo/GAZ_00056797">
        <rdf:type rdf:resource="http://purl.obolibrary.org/obo/ENVO_00000106"/>
        <obo:RO_0001025 rdf:resource="http://purl.obolibrary.org/obo/GAZ_00051914"/>
        <obo:IAO_0000115>A range of the Central Eastern Alps located at the border between Vorarlberg, Liechtenstein and Graubunden. It is the geological border between the Eastern and Western Alps and stretches from the Montafon as far as the Rhine. In the south, the Prattigau is its limit, in the north the Walgau. In the east, it borders the Silvretta groups.</obo:IAO_0000115>
        <oboInOwl:hasOBONamespace>GAZ</oboInOwl:hasOBONamespace>
        <oboInOwl:id>GAZ:00056797</oboInOwl:id>
        <rdfs:label>Ratikon Mountains</rdfs:label>
    </owl:NamedIndividual>
    


    <!-- http://purl.obolibrary.org/obo/GAZ_00056798 -->

    <owl:NamedIndividual rdf:about="http://purl.obolibrary.org/obo/GAZ_00056798">
        <obo:RO_0001025 rdf:resource="http://purl.obolibrary.org/obo/GAZ_00051915"/>
        <obo:IAO_0000115>A group of mountains in Austria, part of the Northern Limestone Alps, lying between the Salzkammergut and the Ennstaler Alpen.</obo:IAO_0000115>
        <oboInOwl:hasOBONamespace>GAZ</oboInOwl:hasOBONamespace>
        <oboInOwl:id>GAZ:00056798</oboInOwl:id>
        <rdfs:label>Totes Gebirge</rdfs:label>
    </owl:NamedIndividual>
    


    <!-- http://purl.obolibrary.org/obo/GAZ_00056799 -->

    <owl:NamedIndividual rdf:about="http://purl.obolibrary.org/obo/GAZ_00056799">
        <obo:RO_0001025 rdf:resource="http://purl.obolibrary.org/obo/GAZ_00051915"/>
        <obo:IAO_0000115>A part of the Northern Limestone Alps. Le massif est entoure par les Alpes d&apos;Ammergau au nord-est, le Wetterstein a l&apos;est, les Alpes de l&apos;Otztal au sud-est, les massifs de Samnaun et de Verwall au sud, le massif de Lechquellen au sud-ouest et les Alpes d&apos;Allgau au nord-ouest. Il est compris entre le Lech au nord-ouest et l&apos;Inn et ses affluents au sud-est.</obo:IAO_0000115>
        <oboInOwl:hasOBONamespace>GAZ</oboInOwl:hasOBONamespace>
        <oboInOwl:id>GAZ:00056799</oboInOwl:id>
        <rdfs:label>Lechtal Alps</rdfs:label>
    </owl:NamedIndividual>
    


    <!-- http://purl.obolibrary.org/obo/GAZ_00056800 -->

    <owl:NamedIndividual rdf:about="http://purl.obolibrary.org/obo/GAZ_00056800">
        <obo:RO_0001025 rdf:resource="http://purl.obolibrary.org/obo/GAZ_00051915"/>
        <obo:IAO_0000115>A mountain range in the Alps, located in Bavaria in Germany and Tyrol and Vorarlberg in Austria.</obo:IAO_0000115>
        <oboInOwl:hasOBONamespace>GAZ</oboInOwl:hasOBONamespace>
        <oboInOwl:id>GAZ:00056800</oboInOwl:id>
        <rdfs:label>Allgau Alps</rdfs:label>
    </owl:NamedIndividual>
    


    <!-- http://purl.obolibrary.org/obo/GAZ_00056801 -->

    <owl:NamedIndividual rdf:about="http://purl.obolibrary.org/obo/GAZ_00056801">
        <obo:RO_0001025 rdf:resource="http://purl.obolibrary.org/obo/GAZ_00051916"/>
        <obo:IAO_0000115>A mountain range in the Italian Alps. It is part of the Southern Limestone Alps. It is located in the provinces of Trento and Brescia. The name stems from its highest peaks: Adamello and Presanella. The Adamello-Presanella Group is separated from the Ortler Alps in the north by the Tonale Pass; from the Bergamo Alps in the west by the Oglio valley (Val Camonica); from the Brenta Group in the east by the Campo Carlo Magno Pass and the river Sarca; to the south it continues towards Lake Iseo.</obo:IAO_0000115>
        <oboInOwl:hasOBONamespace>GAZ</oboInOwl:hasOBONamespace>
        <oboInOwl:id>GAZ:00056801</oboInOwl:id>
        <rdfs:label>Massif de Adamello-Presanella</rdfs:label>
    </owl:NamedIndividual>
    


    <!-- http://purl.obolibrary.org/obo/GAZ_00056802 -->

    <owl:NamedIndividual rdf:about="http://purl.obolibrary.org/obo/GAZ_00056802">
        <obo:RO_0001025 rdf:resource="http://purl.obolibrary.org/obo/GAZ_00051915"/>
        <obo:IAO_0000115>A mountain range in the Northern Limestone Alps. They are located in the Austrian states of Styria and Upper Austria, but mostly in Styria.</obo:IAO_0000115>
        <oboInOwl:hasOBONamespace>GAZ</oboInOwl:hasOBONamespace>
        <oboInOwl:id>GAZ:00056802</oboInOwl:id>
        <rdfs:label>Ennstaler Alps</rdfs:label>
    </owl:NamedIndividual>
    


    <!-- http://purl.obolibrary.org/obo/GAZ_00056803 -->

    <owl:NamedIndividual rdf:about="http://purl.obolibrary.org/obo/GAZ_00056803">
        <obo:RO_0001025 rdf:resource="http://purl.obolibrary.org/obo/GAZ_00051915"/>
        <obo:IAO_0000115>The largest range of the Northern Limestone Alps. Four chains stretch from west to east; in addition, there are a number of fringe ranges and an extensive promontory in the north.</obo:IAO_0000115>
        <oboInOwl:hasOBONamespace>GAZ</oboInOwl:hasOBONamespace>
        <oboInOwl:id>GAZ:00056803</oboInOwl:id>
        <rdfs:label>Karwendel</rdfs:label>
    </owl:NamedIndividual>
    


    <!-- http://purl.obolibrary.org/obo/GAZ_00056804 -->

    <owl:NamedIndividual rdf:about="http://purl.obolibrary.org/obo/GAZ_00056804">
        <obo:RO_0001025 rdf:resource="http://purl.obolibrary.org/obo/GAZ_00378650"/>
        <obo:IAO_0000115>A mountain range that is part of the Southern Limestone Alps in north Slovenia and at the border of Austria. The Kamnik Alps are located at the border of Austria and Slovenia, between the rivers Sava and Savinja.</obo:IAO_0000115>
        <oboInOwl:hasOBONamespace>GAZ</oboInOwl:hasOBONamespace>
        <oboInOwl:id>GAZ:00056804</oboInOwl:id>
        <rdfs:label>Kamnik Alps</rdfs:label>
    </owl:NamedIndividual>
    


    <!-- http://purl.obolibrary.org/obo/GAZ_00056805 -->

    <owl:NamedIndividual rdf:about="http://purl.obolibrary.org/obo/GAZ_00056805">
        <obo:RO_0001025 rdf:resource="http://purl.obolibrary.org/obo/GAZ_00051916"/>
        <obo:IAO_0000115>A part of the Alps that stretch from north-eastern Italy to Slovenia, where they rise to 2864 m at Triglav.</obo:IAO_0000115>
        <oboInOwl:hasOBONamespace>GAZ</oboInOwl:hasOBONamespace>
        <oboInOwl:id>GAZ:00056805</oboInOwl:id>
        <rdfs:label>Julian Alps</rdfs:label>
    </owl:NamedIndividual>
    


    <!-- http://purl.obolibrary.org/obo/GAZ_00056806 -->

    <owl:NamedIndividual rdf:about="http://purl.obolibrary.org/obo/GAZ_00056806">
        <obo:RO_0001025 rdf:resource="http://purl.obolibrary.org/obo/GAZ_00051916"/>
        <obo:IAO_0000115>A mountain range that is located 70% in the provinces of Belluno, the rest in the provinces of Bolzano-Bozen, and Trento (all in north-eastern Italy) and extend from the Adige river in the west to the Piave valley (Pieve di Cadore) in the east. The northern and southern borders are defined by the Puster Valley (Val Pusteria) and the Sugana Valley (Val Sugana).</obo:IAO_0000115>
        <oboInOwl:hasOBONamespace>GAZ</oboInOwl:hasOBONamespace>
        <oboInOwl:id>GAZ:00056806</oboInOwl:id>
        <rdfs:label>Dolomites</rdfs:label>
    </owl:NamedIndividual>
    


    <!-- http://purl.obolibrary.org/obo/GAZ_00056807 -->

    <owl:NamedIndividual rdf:about="http://purl.obolibrary.org/obo/GAZ_00056807">
        <obo:RO_0001025 rdf:resource="http://purl.obolibrary.org/obo/GAZ_00062486"/>
        <obo:IAO_0000115>A national park located in Slovenia. Mt. Triglav is situated almost in the middle of the national park. From it the valleys spread out radially, supplying water to two large river systems which have their sources in the Julian Alps: the Soca and the Sava, flowing to the Adriatic and Black Sea, respectively.</obo:IAO_0000115>
        <oboInOwl:hasOBONamespace>GAZ</oboInOwl:hasOBONamespace>
        <oboInOwl:id>GAZ:00056807</oboInOwl:id>
        <rdfs:label>Triglav National Park</rdfs:label>
    </owl:NamedIndividual>
    


    <!-- http://purl.obolibrary.org/obo/GAZ_00056808 -->

    <owl:NamedIndividual rdf:about="http://purl.obolibrary.org/obo/GAZ_00056808">
        <obo:RO_0001025 rdf:resource="http://purl.obolibrary.org/obo/GAZ_00051916"/>
        <obo:IAO_0000115>A mountain range in the central Alps of Italy. They are considered to be part of the Central Eastern Alps or the Southern Limestone Alps The Ortler Alps are separated from the Livigno Range in the north-west by the Stelvio Pass and the Adda River valley (Valtellina); from the Adamello-Presanella range in the south by the Tonale Pass; from the Otztal Alps in the north-east by the upper Adige valley (Vinschgau-Val Venosta). The part west of the Gavia Pass is also called Sobretta-Gavia Group.</obo:IAO_0000115>
        <oboInOwl:hasOBONamespace>GAZ</oboInOwl:hasOBONamespace>
        <oboInOwl:id>GAZ:00056808</oboInOwl:id>
        <rdfs:label>Ortler Alps</rdfs:label>
    </owl:NamedIndividual>
    


    <!-- http://purl.obolibrary.org/obo/GAZ_00056809 -->

    <owl:NamedIndividual rdf:about="http://purl.obolibrary.org/obo/GAZ_00056809">
        <obo:RO_0001025 rdf:resource="http://purl.obolibrary.org/obo/GAZ_00051916"/>
        <obo:IAO_0000115>A mountain range on the border between Slovenia and Austria. With a total length of 120 km, the Karawanken chain is the longest range in Europe. Together with the Kamnik Alps and the Savinja Alps, the Karawanken chain forms a natural border between Austria and Slovenia.</obo:IAO_0000115>
        <oboInOwl:hasOBONamespace>GAZ</oboInOwl:hasOBONamespace>
        <oboInOwl:id>GAZ:00056809</oboInOwl:id>
        <rdfs:label>Karawanken</rdfs:label>
    </owl:NamedIndividual>
    


    <!-- http://purl.obolibrary.org/obo/GAZ_00056810 -->

    <owl:NamedIndividual rdf:about="http://purl.obolibrary.org/obo/GAZ_00056810">
        <obo:RO_0001025 rdf:resource="http://purl.obolibrary.org/obo/GAZ_00060609"/>
        <obo:IAO_0000115>A mountain range in central Switzerland in the western part of the Alps. They extend into the cantons of Obwalden, Valais, Lucerne, Bern, Uri and Nidwalden and are bordered by the Bernese Alps to the west, the Lepontine Alps to the south and the Glarus Alps to the east.</obo:IAO_0000115>
        <oboInOwl:hasOBONamespace>GAZ</oboInOwl:hasOBONamespace>
        <oboInOwl:id>GAZ:00056810</oboInOwl:id>
        <rdfs:label>Urner Alps</rdfs:label>
    </owl:NamedIndividual>
    


    <!-- http://purl.obolibrary.org/obo/GAZ_00056811 -->

    <owl:NamedIndividual rdf:about="http://purl.obolibrary.org/obo/GAZ_00056811">
        <obo:RO_0001025 rdf:resource="http://purl.obolibrary.org/obo/GAZ_00060581"/>
        <obo:IAO_0000115>A mountain range situated in the Chablais valaisan in Chablais, in the Canton of Valais, Switzerland. Its reaches a height of 3,257 m. Dominating the Val-d&apos;Illiez and the Rhone Valley, to the south they face the Lac de Salanfe, an artificial reservoir. Geologically they make up a part of the massif Haut-Giffre.</obo:IAO_0000115>
        <oboInOwl:hasOBONamespace>GAZ</oboInOwl:hasOBONamespace>
        <oboInOwl:id>GAZ:00056811</oboInOwl:id>
        <rdfs:label>Dents du Midi</rdfs:label>
    </owl:NamedIndividual>
    


    <!-- http://purl.obolibrary.org/obo/GAZ_00057281 -->

    <owl:NamedIndividual rdf:about="http://purl.obolibrary.org/obo/GAZ_00057281">
        <obo:RO_0001025 rdf:resource="http://purl.obolibrary.org/obo/GAZ_00056788"/>
        <obo:IAO_0000115>A mountain range in the Alps of eastern Switzerland and northern Italy, around the Italian village Livigno. It is considered to be part of the Central Eastern Alps. The Livigno Range is separated from the Bernina Range in the south-west by the Bernina Pass; from the Albula Range in the north-west by the Upper Engadin valley; from the Sesvenna Range in the north-east by the Ofen Pass and Val Mustair; from the Ortler Alps in the east by the upper Adda River valley (Valtellina) and the Stelvio Pass.</obo:IAO_0000115>
        <oboInOwl:hasOBONamespace>GAZ</oboInOwl:hasOBONamespace>
        <oboInOwl:id>GAZ:00057281</oboInOwl:id>
        <rdfs:label>Livigno Range</rdfs:label>
    </owl:NamedIndividual>
    


    <!-- http://purl.obolibrary.org/obo/GAZ_00057282 -->

    <owl:NamedIndividual rdf:about="http://purl.obolibrary.org/obo/GAZ_00057282">
        <obo:RO_0001025 rdf:resource="http://purl.obolibrary.org/obo/GAZ_00056788"/>
        <obo:IAO_0000115>A mountain range in the Alps of eastern Switzerland and northern Italy. It is considered to be part of the Central Eastern Alps. The Oberhalbstein Range is separated from the Lepontine Alps in the west by the Splugen Pass; from the Plessur Range in the north by the Albula river valley; from the Albula Range in the east by the Septimer Pass and the Julia River; from the Bernina Range in the south by the Val Bregaglia. The Oberhalbstein Range is drained by the rivers Hinterrhein, Julia, Liro and Mera.</obo:IAO_0000115>
        <oboInOwl:hasOBONamespace>GAZ</oboInOwl:hasOBONamespace>
        <oboInOwl:id>GAZ:00057282</oboInOwl:id>
        <rdfs:label>Oberhalbstein Range</rdfs:label>
    </owl:NamedIndividual>
    


    <!-- http://purl.obolibrary.org/obo/GAZ_00057283 -->

    <owl:NamedIndividual rdf:about="http://purl.obolibrary.org/obo/GAZ_00057283">
        <obo:RO_0001025 rdf:resource="http://purl.obolibrary.org/obo/GAZ_00056788"/>
        <obo:IAO_0000115>A mountain range in the Alps of eastern Switzerland. It is considered to be part of the Central Eastern Alps. The Albula Range is separated from the Oberhalbstein Range in the west by the Septimer Pass and the Julia River valley; from the Plessur Range in the north-west by the Landwasser river valley; from the Silvretta group in the north-east by the Fluela Pass; from the Bernina Range in the south-east by the Maloja Pass and the Inn River valley (upper Engadin). The Albula Range is drained by the Albula, Julia, Landwasser and Inn rivers.</obo:IAO_0000115>
        <oboInOwl:hasOBONamespace>GAZ</oboInOwl:hasOBONamespace>
        <oboInOwl:id>GAZ:00057283</oboInOwl:id>
        <rdfs:label>Albula Range</rdfs:label>
    </owl:NamedIndividual>
    


    <!-- http://purl.obolibrary.org/obo/GAZ_00057284 -->

    <owl:NamedIndividual rdf:about="http://purl.obolibrary.org/obo/GAZ_00057284">
        <obo:RO_0001025 rdf:resource="http://purl.obolibrary.org/obo/GAZ_00056788"/>
        <obo:IAO_0000115>A mountain range of the Central Eastern Alps shared by Tirol, Vorarlberg (both in Austria) and Graubunden (Switzerland). The Silvretta is surrounded by the Ratikon, Verwall and Samnaun ranges.</obo:IAO_0000115>
        <oboInOwl:hasOBONamespace>GAZ</oboInOwl:hasOBONamespace>
        <oboInOwl:id>GAZ:00057284</oboInOwl:id>
        <rdfs:label>Silvretta Range</rdfs:label>
    </owl:NamedIndividual>
    


    <!-- http://purl.obolibrary.org/obo/GAZ_00057285 -->

    <owl:NamedIndividual rdf:about="http://purl.obolibrary.org/obo/GAZ_00057285">
        <obo:RO_0001025 rdf:resource="http://purl.obolibrary.org/obo/GAZ_00056788"/>
        <obo:IAO_0000115>A mountain range in the Alps of eastern Switzerland. It is considered to be part of the Central Eastern Alps. It is named after the river Plessur, which originates from the center of the range. The Plessur Range is separated from the Glarus Alps in the west by the Rhine valley; from the Ratikon range in the north by the Landquart river valley (Prattigau); from the Albula Range in the south-east by the Landwasser river valley; from the Oberhalbstein Range in the south by the Albula river valley. The Plessur Range is drained by the rivers Rhine, Plessur, Landwasser and Landquart.</obo:IAO_0000115>
        <oboInOwl:hasOBONamespace>GAZ</oboInOwl:hasOBONamespace>
        <oboInOwl:id>GAZ:00057285</oboInOwl:id>
        <rdfs:label>Plessur Range</rdfs:label>
    </owl:NamedIndividual>
    


    <!-- http://purl.obolibrary.org/obo/GAZ_00057286 -->

    <owl:NamedIndividual rdf:about="http://purl.obolibrary.org/obo/GAZ_00057286">
        <obo:RO_0001025 rdf:resource="http://purl.obolibrary.org/obo/GAZ_00056788"/>
        <obo:IAO_0000115>A mountain range of the Central Eastern Alps located at the border of Tirol and Graubunden.</obo:IAO_0000115>
        <oboInOwl:hasOBONamespace>GAZ</oboInOwl:hasOBONamespace>
        <oboInOwl:id>GAZ:00057286</oboInOwl:id>
        <rdfs:label>Samnaun Alps</rdfs:label>
    </owl:NamedIndividual>
    


    <!-- http://purl.obolibrary.org/obo/GAZ_00057287 -->

    <owl:NamedIndividual rdf:about="http://purl.obolibrary.org/obo/GAZ_00057287">
        <obo:RO_0001025 rdf:resource="http://purl.obolibrary.org/obo/GAZ_00056788"/>
        <obo:IAO_0000115>A mountain range in the Alps of eastern Switzerland and northern Italy. It is considered to be part of the Central Eastern Alps. The Bernina Range is separated from the Albula Range in the north-west by the Maloja Pass and the Upper Engadin valley; from the Livigno Range in the east by the Bernina Pass; from the Bergamo Alps in the south by the Adda valley (Valtellina); and from the Bregaglia Range in the south-west by the Muretto Pass. The Bernina Range is drained by the rivers Adda, Inn and Maira (Mera in Italy).</obo:IAO_0000115>
        <oboInOwl:hasOBONamespace>GAZ</oboInOwl:hasOBONamespace>
        <oboInOwl:id>GAZ:00057287</oboInOwl:id>
        <rdfs:label>Bernina Range</rdfs:label>
    </owl:NamedIndividual>
    


    <!-- http://purl.obolibrary.org/obo/GAZ_00057288 -->

    <owl:NamedIndividual rdf:about="http://purl.obolibrary.org/obo/GAZ_00057288">
        <obo:RO_0001025 rdf:resource="http://purl.obolibrary.org/obo/GAZ_00056788"/>
        <obo:IAO_0000115>A small group of mostly granite mountains in Graubunden, Switzerland and Sondrio, Italy.</obo:IAO_0000115>
        <oboInOwl:hasOBONamespace>GAZ</oboInOwl:hasOBONamespace>
        <oboInOwl:id>GAZ:00057288</oboInOwl:id>
        <rdfs:label>Bregaglia Range</rdfs:label>
    </owl:NamedIndividual>
    


    <!-- http://purl.obolibrary.org/obo/GAZ_00057289 -->

    <owl:NamedIndividual rdf:about="http://purl.obolibrary.org/obo/GAZ_00057289">
        <obo:RO_0001025 rdf:resource="http://purl.obolibrary.org/obo/GAZ_00056788"/>
        <obo:IAO_0000115>A mountain range in the Alps of eastern Switzerland and northern Italy. It is considered to be part of the Central Eastern Alps. The Sesvenna Range is separated from the Silvretta Group in the north and the Albula Range in the west by the Lower Engadin valley; from the Livigno Range in the south-west by the Ofen Pass and Val Mustair; from the Otztal Alps in the east by the upper Adige valley and the Reschen Pass. The Sesvenna Range is drained by the rivers Inn and Adige.</obo:IAO_0000115>
        <oboInOwl:hasOBONamespace>GAZ</oboInOwl:hasOBONamespace>
        <oboInOwl:id>GAZ:00057289</oboInOwl:id>
        <rdfs:label>Sesvenna Range</rdfs:label>
    </owl:NamedIndividual>
    


    <!-- http://purl.obolibrary.org/obo/GAZ_00058601 -->

    <owl:NamedIndividual rdf:about="http://purl.obolibrary.org/obo/GAZ_00058601">
        <obo:RO_0001025 rdf:resource="http://purl.obolibrary.org/obo/GAZ_00056790"/>
        <obo:IAO_0000115>A lake in Tyrol, Austria. It lies northern above the village Obernberg am Brenner on 2.100 m above sea level.</obo:IAO_0000115>
        <oboInOwl:hasOBONamespace>GAZ</oboInOwl:hasOBONamespace>
        <oboInOwl:id>GAZ:00058601</oboInOwl:id>
        <rdfs:label>Lichtsee</rdfs:label>
    </owl:NamedIndividual>
    


    <!-- http://purl.obolibrary.org/obo/GAZ_00058608 -->

    <owl:NamedIndividual rdf:about="http://purl.obolibrary.org/obo/GAZ_00058608">
        <obo:RO_0001025 rdf:resource="http://purl.obolibrary.org/obo/GAZ_00056790"/>
        <obo:IAO_0000115>A lake that lies N of the village Obernberg am Brenner on 2070 m above sea level.</obo:IAO_0000115>
        <oboInOwl:hasOBONamespace>GAZ</oboInOwl:hasOBONamespace>
        <oboInOwl:id>GAZ:00058608</oboInOwl:id>
        <rdfs:label>Rohrsee</rdfs:label>
    </owl:NamedIndividual>
    


    <!-- http://purl.obolibrary.org/obo/GAZ_00058614 -->

    <owl:NamedIndividual rdf:about="http://purl.obolibrary.org/obo/GAZ_00058614">
        <obo:RO_0001025 rdf:resource="http://purl.obolibrary.org/obo/GAZ_00056798"/>
        <obo:IAO_0000115>A lake in Upper Austria in the Almtal valley, south of the town of Grunau im Almtal. The lake lies in the northern portion of the Totes Gebirge mountains and is about 2.3 km by 700 m wide.</obo:IAO_0000115>
        <oboInOwl:hasOBONamespace>GAZ</oboInOwl:hasOBONamespace>
        <oboInOwl:id>GAZ:00058614</oboInOwl:id>
        <rdfs:label>Almsee</rdfs:label>
    </owl:NamedIndividual>
    


    <!-- http://purl.obolibrary.org/obo/GAZ_00058616 -->

    <owl:NamedIndividual rdf:about="http://purl.obolibrary.org/obo/GAZ_00058616">
        <obo:RO_0001025 rdf:resource="http://purl.obolibrary.org/obo/GAZ_00008111"/>
        <obo:IAO_0000115>The W part of the Bodensee.</obo:IAO_0000115>
        <oboInOwl:hasOBONamespace>GAZ</oboInOwl:hasOBONamespace>
        <oboInOwl:id>GAZ:00058616</oboInOwl:id>
        <rdfs:label>Untersee</rdfs:label>
    </owl:NamedIndividual>
    


    <!-- http://purl.obolibrary.org/obo/GAZ_00058617 -->

    <owl:NamedIndividual rdf:about="http://purl.obolibrary.org/obo/GAZ_00058617">
        <obo:RO_0001025 rdf:resource="http://purl.obolibrary.org/obo/GAZ_00008111"/>
        <obo:IAO_0000115>The N part of the Bodensee.</obo:IAO_0000115>
        <oboInOwl:hasOBONamespace>GAZ</oboInOwl:hasOBONamespace>
        <oboInOwl:id>GAZ:00058617</oboInOwl:id>
        <rdfs:label>Uberlinger See</rdfs:label>
    </owl:NamedIndividual>
    


    <!-- http://purl.obolibrary.org/obo/GAZ_00058618 -->

    <owl:NamedIndividual rdf:about="http://purl.obolibrary.org/obo/GAZ_00058618">
        <obo:RO_0001025 rdf:resource="http://purl.obolibrary.org/obo/GAZ_00008111"/>
        <obo:IAO_0000115>The main part of the Bodensee.</obo:IAO_0000115>
        <oboInOwl:hasOBONamespace>GAZ</oboInOwl:hasOBONamespace>
        <oboInOwl:id>GAZ:00058618</oboInOwl:id>
        <rdfs:label>Obersee</rdfs:label>
    </owl:NamedIndividual>
    


    <!-- http://purl.obolibrary.org/obo/GAZ_00058619 -->

    <owl:NamedIndividual rdf:about="http://purl.obolibrary.org/obo/GAZ_00058619">
        <obo:RO_0001025 rdf:resource="http://purl.obolibrary.org/obo/GAZ_00008111"/>
        <obo:IAO_0000115>The NW part of the Bodensee.</obo:IAO_0000115>
        <oboInOwl:hasOBONamespace>GAZ</oboInOwl:hasOBONamespace>
        <oboInOwl:id>GAZ:00058619</oboInOwl:id>
        <rdfs:label>Gnadensee</rdfs:label>
    </owl:NamedIndividual>
    


    <!-- http://purl.obolibrary.org/obo/GAZ_00058626 -->

    <owl:NamedIndividual rdf:about="http://purl.obolibrary.org/obo/GAZ_00058626">
        <obo:RO_0001025 rdf:resource="http://purl.obolibrary.org/obo/GAZ_00056799"/>
        <obo:IAO_0000115>A lake SW of the village Egg in Vorarlberg at 1600 m in Austria. It lies within the &quot;Lechtaler&quot; Alps in Vorarlberg.</obo:IAO_0000115>
        <oboInOwl:hasOBONamespace>GAZ</oboInOwl:hasOBONamespace>
        <oboInOwl:id>GAZ:00058626</oboInOwl:id>
        <rdfs:label>Korbersee</rdfs:label>
    </owl:NamedIndividual>
    


    <!-- http://purl.obolibrary.org/obo/GAZ_00058631 -->

    <owl:NamedIndividual rdf:about="http://purl.obolibrary.org/obo/GAZ_00058631">
        <obo:RO_0001025 rdf:resource="http://purl.obolibrary.org/obo/GAZ_00051914"/>
        <obo:IAO_0000115>A glacial meromictic lake in the Central Eastern Alps, near the town of Spittal an der Drau.</obo:IAO_0000115>
        <oboInOwl:hasOBONamespace>GAZ</oboInOwl:hasOBONamespace>
        <oboInOwl:id>GAZ:00058631</oboInOwl:id>
        <rdfs:label>Millstatter See</rdfs:label>
    </owl:NamedIndividual>
    


    <!-- http://purl.obolibrary.org/obo/GAZ_00058632 -->

    <owl:NamedIndividual rdf:about="http://purl.obolibrary.org/obo/GAZ_00058632">
        <obo:RO_0001025 rdf:resource="http://purl.obolibrary.org/obo/GAZ_00060642"/>
        <obo:IAO_0000115>A lake in the Upper Austrian part of the Salzkammergut and neighbour to the larger Attersee. Its southwestern shore marks the border between the states of Upper Austria and Salzburg, and also between the Northern Limestone Alps in the South and the Sandstone zone of the Northern Alps.</obo:IAO_0000115>
        <oboInOwl:hasOBONamespace>GAZ</oboInOwl:hasOBONamespace>
        <oboInOwl:id>GAZ:00058632</oboInOwl:id>
        <rdfs:label>Mondsee</rdfs:label>
    </owl:NamedIndividual>
    


    <!-- http://purl.obolibrary.org/obo/GAZ_00058638 -->

    <owl:NamedIndividual rdf:about="http://purl.obolibrary.org/obo/GAZ_00058638">
        <obo:RO_0001025 rdf:resource="http://purl.obolibrary.org/obo/GAZ_00060642"/>
        <obo:IAO_0000115>A lake in the Salzkammergut, Austria.</obo:IAO_0000115>
        <oboInOwl:hasOBONamespace>GAZ</oboInOwl:hasOBONamespace>
        <oboInOwl:id>GAZ:00058638</oboInOwl:id>
        <rdfs:label>Traunsee</rdfs:label>
    </owl:NamedIndividual>
    


    <!-- http://purl.obolibrary.org/obo/GAZ_00058641 -->

    <owl:NamedIndividual rdf:about="http://purl.obolibrary.org/obo/GAZ_00058641">
        <obo:RO_0001025 rdf:resource="http://purl.obolibrary.org/obo/GAZ_00056798"/>
        <obo:IAO_0000115>A lake in Upper Austria in the Salzkammergut resort region.</obo:IAO_0000115>
        <oboInOwl:hasOBONamespace>GAZ</oboInOwl:hasOBONamespace>
        <oboInOwl:id>GAZ:00058641</oboInOwl:id>
        <rdfs:label>Wildensee</rdfs:label>
    </owl:NamedIndividual>
    


    <!-- http://purl.obolibrary.org/obo/GAZ_00058642 -->

    <owl:NamedIndividual rdf:about="http://purl.obolibrary.org/obo/GAZ_00058642">
        <obo:RO_0001025 rdf:resource="http://purl.obolibrary.org/obo/GAZ_00060642"/>
        <obo:IAO_0000115>A lake located mostly within the State of Salzburg. The W part is known as the Abersee.</obo:IAO_0000115>
        <oboInOwl:hasOBONamespace>GAZ</oboInOwl:hasOBONamespace>
        <oboInOwl:id>GAZ:00058642</oboInOwl:id>
        <rdfs:label>Wolfgangsee</rdfs:label>
    </owl:NamedIndividual>
    


    <!-- http://purl.obolibrary.org/obo/GAZ_00058643 -->

    <owl:NamedIndividual rdf:about="http://purl.obolibrary.org/obo/GAZ_00058643">
        <obo:RO_0001025 rdf:resource="http://purl.obolibrary.org/obo/GAZ_00058642"/>
        <obo:IAO_0000115>The W part of the Wolfgangsee.</obo:IAO_0000115>
        <oboInOwl:hasOBONamespace>GAZ</oboInOwl:hasOBONamespace>
        <oboInOwl:id>GAZ:00058643</oboInOwl:id>
        <rdfs:label>Abersee</rdfs:label>
    </owl:NamedIndividual>
    


    <!-- http://purl.obolibrary.org/obo/GAZ_00058644 -->

    <owl:NamedIndividual rdf:about="http://purl.obolibrary.org/obo/GAZ_00058644">
        <obo:RO_0001025 rdf:resource="http://purl.obolibrary.org/obo/GAZ_00060642"/>
        <obo:IAO_0000115>A small freshwater lake in the Austrian Alps. The lake is fed by numerous small mountain streams in summer, but only one stream flows out of it into the river Salzach.</obo:IAO_0000115>
        <oboInOwl:hasOBONamespace>GAZ</oboInOwl:hasOBONamespace>
        <oboInOwl:id>GAZ:00058644</oboInOwl:id>
        <rdfs:label>Zeller See</rdfs:label>
    </owl:NamedIndividual>
    


    <!-- http://purl.obolibrary.org/obo/GAZ_00058898 -->

    <owl:NamedIndividual rdf:about="http://purl.obolibrary.org/obo/GAZ_00058898">
        <obo:RO_0001025 rdf:resource="http://purl.obolibrary.org/obo/GAZ_00144376"/>
        <obo:IAO_0000115>A former Rhine-Meuse estuary on the border of the Dutch provinces of South Holland and Zeeland that has become a lake due to the Delta Works. It is situated between the former islands of Goeree-Overflakkee (South Holland) and Schouwen-Duiveland (Zeeland) which are connected by the Brouwersdam on the west and the Grevelingendam on the east.</obo:IAO_0000115>
        <oboInOwl:hasOBONamespace>GAZ</oboInOwl:hasOBONamespace>
        <oboInOwl:id>GAZ:00058898</oboInOwl:id>
        <rdfs:label>Grevelingen</rdfs:label>
    </owl:NamedIndividual>
    


    <!-- http://purl.obolibrary.org/obo/GAZ_00058902 -->

    <owl:NamedIndividual rdf:about="http://purl.obolibrary.org/obo/GAZ_00058902">
        <obo:IAO_0000115>A river, formerly a bay, in the Dutch province of North Holland. The waterfront of Amsterdam. In historic times, the IJ was a long and narrow brackish bay that connected to the Zuiderzee (itself a bay of the North Sea) and stretched from Amsterdam in the east to Velsen in the west.</obo:IAO_0000115>
        <oboInOwl:hasOBONamespace>GAZ</oboInOwl:hasOBONamespace>
        <oboInOwl:id>GAZ:00058902</oboInOwl:id>
        <rdfs:label>IJ</rdfs:label>
    </owl:NamedIndividual>
    


    <!-- http://purl.obolibrary.org/obo/GAZ_00058955 -->

    <owl:NamedIndividual rdf:about="http://purl.obolibrary.org/obo/GAZ_00058955">
        <obo:RO_0001025 rdf:resource="http://purl.obolibrary.org/obo/GAZ_00056805"/>
        <obo:IAO_0000115>A glacial lake in the Julian Alps in northwestern Slovenia, where it adjoins the town of Bled.</obo:IAO_0000115>
        <oboInOwl:hasOBONamespace>GAZ</oboInOwl:hasOBONamespace>
        <oboInOwl:id>GAZ:00058955</oboInOwl:id>
        <rdfs:label>Lake Bled</rdfs:label>
    </owl:NamedIndividual>
    


    <!-- http://purl.obolibrary.org/obo/GAZ_00058956 -->

    <owl:NamedIndividual rdf:about="http://purl.obolibrary.org/obo/GAZ_00058956">
        <obo:RO_0001025 rdf:resource="http://purl.obolibrary.org/obo/GAZ_00058955"/>
        <obo:IAO_0000115>An island in Lake Bled.</obo:IAO_0000115>
        <oboInOwl:hasOBONamespace>GAZ</oboInOwl:hasOBONamespace>
        <oboInOwl:id>GAZ:00058956</oboInOwl:id>
        <rdfs:label>Blejski otok</rdfs:label>
    </owl:NamedIndividual>
    


    <!-- http://purl.obolibrary.org/obo/GAZ_00059213 -->

    <owl:NamedIndividual rdf:about="http://purl.obolibrary.org/obo/GAZ_00059213">
        <obo:RO_0001025 rdf:resource="http://purl.obolibrary.org/obo/GAZ_00059214"/>
        <obo:IAO_0000115>A lake in the Grandes Rousses massif of the French Alps.</obo:IAO_0000115>
        <oboInOwl:hasOBONamespace>GAZ</oboInOwl:hasOBONamespace>
        <oboInOwl:id>GAZ:00059213</oboInOwl:id>
        <rdfs:label>Lac Bramant</rdfs:label>
    </owl:NamedIndividual>
    


    <!-- http://purl.obolibrary.org/obo/GAZ_00059214 -->

    <owl:NamedIndividual rdf:about="http://purl.obolibrary.org/obo/GAZ_00059214">
        <obo:RO_0001025 rdf:resource="http://purl.obolibrary.org/obo/GAZ_00009675"/>
        <obo:IAO_0000115>A massif in the Dauphine Alps.</obo:IAO_0000115>
        <oboInOwl:hasOBONamespace>GAZ</oboInOwl:hasOBONamespace>
        <oboInOwl:id>GAZ:00059214</oboInOwl:id>
        <rdfs:label>Grandes Rousses</rdfs:label>
    </owl:NamedIndividual>
    


    <!-- http://purl.obolibrary.org/obo/GAZ_00059234 -->

    <owl:NamedIndividual rdf:about="http://purl.obolibrary.org/obo/GAZ_00059234">
        <obo:RO_0001025 rdf:resource="http://purl.obolibrary.org/obo/GAZ_00059236"/>
        <obo:IAO_0000115>One of the Laffrey lakes, located in Matheysine at 23km south of Grenoble, in the Isere departement.</obo:IAO_0000115>
        <oboInOwl:hasOBONamespace>GAZ</oboInOwl:hasOBONamespace>
        <oboInOwl:id>GAZ:00059234</oboInOwl:id>
        <rdfs:label>Grand lac de Laffrey</rdfs:label>
    </owl:NamedIndividual>
    


    <!-- http://purl.obolibrary.org/obo/GAZ_00059235 -->

    <owl:NamedIndividual rdf:about="http://purl.obolibrary.org/obo/GAZ_00059235">
        <obo:RO_0001025 rdf:resource="http://purl.obolibrary.org/obo/GAZ_00059237"/>
        <obo:IAO_0000115>A region located in the Alps in the south of the Isere departement. It is a plateau surroundered by mountains. It roughly matches the boundaries of the canton of La Mure. It is around 20 km long from north to south and around 13km wide from east to west. At the south and at the west, the border of the plateau is marked by the Drac River, which defines the boundary with Trieves (at the south) and with the Vercors Plateau (at the west). At the north, the plateau ends at the Laffrey slope down to the Romanche valley at the elevation of 350m. At the east, the small mountain range including the summits of Grand Serre (elev. 2,141 m) and Tabor (elev. 2,389 m) marks the boundary with the Valbonnais canton.</obo:IAO_0000115>
        <oboInOwl:hasOBONamespace>GAZ</oboInOwl:hasOBONamespace>
        <oboInOwl:id>GAZ:00059235</oboInOwl:id>
        <rdfs:label>Plateau Matheysine</rdfs:label>
    </owl:NamedIndividual>
    


    <!-- http://purl.obolibrary.org/obo/GAZ_00059236 -->

    <owl:NamedIndividual rdf:about="http://purl.obolibrary.org/obo/GAZ_00059236">
        <obo:RO_0001025 rdf:resource="http://purl.obolibrary.org/obo/GAZ_00059235"/>
        <obo:IAO_0000115>Four lakes in the Commune of Laffrey.</obo:IAO_0000115>
        <oboInOwl:hasOBONamespace>GAZ</oboInOwl:hasOBONamespace>
        <oboInOwl:id>GAZ:00059236</oboInOwl:id>
        <rdfs:label>Lacs de Laffrey</rdfs:label>
    </owl:NamedIndividual>
    


    <!-- http://purl.obolibrary.org/obo/GAZ_00059237 -->

    <owl:NamedIndividual rdf:about="http://purl.obolibrary.org/obo/GAZ_00059237">
        <obo:RO_0001025 rdf:resource="http://purl.obolibrary.org/obo/GAZ_00009675"/>
        <obo:IAO_0000115>A small massif of the French Alps in Isere. Il prolonge au sud-ouest la chaine de Belledonne et se situe au nord-ouest du massif des Ecrins, au nord du massif du Devoluy, et a l&apos;est du Vercors. Il est borde par le Drac, la Romanche et la Malsanne.</obo:IAO_0000115>
        <oboInOwl:hasOBONamespace>GAZ</oboInOwl:hasOBONamespace>
        <oboInOwl:id>GAZ:00059237</oboInOwl:id>
        <rdfs:label>Massif du Taillefer</rdfs:label>
    </owl:NamedIndividual>
    


    <!-- http://purl.obolibrary.org/obo/GAZ_00059238 -->

    <owl:NamedIndividual rdf:about="http://purl.obolibrary.org/obo/GAZ_00059238">
        <obo:RO_0001025 rdf:resource="http://purl.obolibrary.org/obo/GAZ_00059236"/>
        <obo:IAO_0000115>One of the Lacs de Laffrey.</obo:IAO_0000115>
        <oboInOwl:hasOBONamespace>GAZ</oboInOwl:hasOBONamespace>
        <oboInOwl:id>GAZ:00059238</oboInOwl:id>
        <rdfs:label>Lac de Petitchet</rdfs:label>
    </owl:NamedIndividual>
    


    <!-- http://purl.obolibrary.org/obo/GAZ_00059239 -->

    <owl:NamedIndividual rdf:about="http://purl.obolibrary.org/obo/GAZ_00059239">
        <obo:RO_0001025 rdf:resource="http://purl.obolibrary.org/obo/GAZ_00059236"/>
        <obo:IAO_0000115>One of the Lacs de Laffrey.</obo:IAO_0000115>
        <oboInOwl:hasOBONamespace>GAZ</oboInOwl:hasOBONamespace>
        <oboInOwl:id>GAZ:00059239</oboInOwl:id>
        <rdfs:label>Lac de Pierre-Chatel</rdfs:label>
    </owl:NamedIndividual>
    


    <!-- http://purl.obolibrary.org/obo/GAZ_00059240 -->

    <owl:NamedIndividual rdf:about="http://purl.obolibrary.org/obo/GAZ_00059240">
        <obo:RO_0001025 rdf:resource="http://purl.obolibrary.org/obo/GAZ_00059236"/>
        <obo:IAO_0000115>One of the Lacs de Laffrey.</obo:IAO_0000115>
        <oboInOwl:hasOBONamespace>GAZ</oboInOwl:hasOBONamespace>
        <oboInOwl:id>GAZ:00059240</oboInOwl:id>
        <rdfs:label>Lac Mort</rdfs:label>
    </owl:NamedIndividual>
    


    <!-- http://purl.obolibrary.org/obo/GAZ_00059269 -->

    <owl:NamedIndividual rdf:about="http://purl.obolibrary.org/obo/GAZ_00059269">
        <obo:IAO_0000115>Un petit lac du versant alsacien des Vosges, d&apos;origine glaciaire. Ses eaux rejoignent la Fecht par un petit affluent gauche, le Wormsabachrunz.</obo:IAO_0000115>
        <oboInOwl:hasOBONamespace>GAZ</oboInOwl:hasOBONamespace>
        <oboInOwl:id>GAZ:00059269</oboInOwl:id>
        <rdfs:label>Lac du Schiessrothried</rdfs:label>
    </owl:NamedIndividual>
    


    <!-- http://purl.obolibrary.org/obo/GAZ_00059753 -->

    <owl:NamedIndividual rdf:about="http://purl.obolibrary.org/obo/GAZ_00059753">
        <obo:IAO_0000115>A man-made lake in the Lorraine Region.</obo:IAO_0000115>
        <oboInOwl:hasOBONamespace>GAZ</oboInOwl:hasOBONamespace>
        <oboInOwl:id>GAZ:00059753</oboInOwl:id>
        <rdfs:label>Lac de Madine</rdfs:label>
    </owl:NamedIndividual>
    


    <!-- http://purl.obolibrary.org/obo/GAZ_00060182 -->

    <owl:NamedIndividual rdf:about="http://purl.obolibrary.org/obo/GAZ_00060182">
        <obo:RO_0001025 rdf:resource="http://purl.obolibrary.org/obo/GAZ_00008405"/>
        <obo:IAO_0000115>A region of the French Alps on the franco-italian border. On the French side it lies in the departements of Hautes-Alpes and Savoie. The massif consists of smaller mountain chains including Mont Thabor as well as those of the Grand Galibier, Mont Chaberton and the Rois Mages. It is bordered by the massif de la Vanoise to the north, the massif du Mont-Cenis to the north-east, the Alpes Cottiennes to the east, the massif du Queyras and Ecrins to the south and the massif d&apos;Arvan-Villards to the west. The northernmost end of the range is bordered by the Arc river to the north in the Maurienne valley, and the Guisane river to the south.</obo:IAO_0000115>
        <oboInOwl:hasOBONamespace>GAZ</oboInOwl:hasOBONamespace>
        <oboInOwl:id>GAZ:00060182</oboInOwl:id>
        <rdfs:label>Massif des Cerces</rdfs:label>
    </owl:NamedIndividual>
    


    <!-- http://purl.obolibrary.org/obo/GAZ_00060193 -->

    <owl:NamedIndividual rdf:about="http://purl.obolibrary.org/obo/GAZ_00060193">
        <obo:RO_0001025 rdf:resource="http://purl.obolibrary.org/obo/GAZ_00060182"/>
        <obo:IAO_0000115>A lake in the Massif des Cerces.</obo:IAO_0000115>
        <oboInOwl:hasOBONamespace>GAZ</oboInOwl:hasOBONamespace>
        <oboInOwl:id>GAZ:00060193</oboInOwl:id>
        <rdfs:label>Grand Lac</rdfs:label>
    </owl:NamedIndividual>
    


    <!-- http://purl.obolibrary.org/obo/GAZ_00060194 -->

    <owl:NamedIndividual rdf:about="http://purl.obolibrary.org/obo/GAZ_00060194">
        <obo:RO_0001025 rdf:resource="http://purl.obolibrary.org/obo/GAZ_00060182"/>
        <obo:IAO_0000115>A lake in the Massif des Cerces.</obo:IAO_0000115>
        <oboInOwl:hasOBONamespace>GAZ</oboInOwl:hasOBONamespace>
        <oboInOwl:id>GAZ:00060194</oboInOwl:id>
        <rdfs:label>Lac des Beraudes</rdfs:label>
    </owl:NamedIndividual>
    


    <!-- http://purl.obolibrary.org/obo/GAZ_00060195 -->

    <owl:NamedIndividual rdf:about="http://purl.obolibrary.org/obo/GAZ_00060195">
        <obo:RO_0001025 rdf:resource="http://purl.obolibrary.org/obo/GAZ_00060182"/>
        <obo:IAO_0000115>A lake in the Massif des Cerces.</obo:IAO_0000115>
        <oboInOwl:hasOBONamespace>GAZ</oboInOwl:hasOBONamespace>
        <oboInOwl:id>GAZ:00060195</oboInOwl:id>
        <rdfs:label>Lac de Cristol</rdfs:label>
    </owl:NamedIndividual>
    


    <!-- http://purl.obolibrary.org/obo/GAZ_00060196 -->

    <owl:NamedIndividual rdf:about="http://purl.obolibrary.org/obo/GAZ_00060196">
        <obo:RO_0001025 rdf:resource="http://purl.obolibrary.org/obo/GAZ_00060182"/>
        <obo:IAO_0000115>A lake in the Massif des Cerces.</obo:IAO_0000115>
        <oboInOwl:hasOBONamespace>GAZ</oboInOwl:hasOBONamespace>
        <oboInOwl:id>GAZ:00060196</oboInOwl:id>
        <rdfs:label>Lac Haut-des-Drayeres</rdfs:label>
    </owl:NamedIndividual>
    


    <!-- http://purl.obolibrary.org/obo/GAZ_00060197 -->

    <owl:NamedIndividual rdf:about="http://purl.obolibrary.org/obo/GAZ_00060197">
        <obo:RO_0001025 rdf:resource="http://purl.obolibrary.org/obo/GAZ_00060182"/>
        <obo:IAO_0000115>A lake in the Massif des Cerces.</obo:IAO_0000115>
        <oboInOwl:hasOBONamespace>GAZ</oboInOwl:hasOBONamespace>
        <oboInOwl:id>GAZ:00060197</oboInOwl:id>
        <rdfs:label>Lac Gimont</rdfs:label>
    </owl:NamedIndividual>
    


    <!-- http://purl.obolibrary.org/obo/GAZ_00060198 -->

    <owl:NamedIndividual rdf:about="http://purl.obolibrary.org/obo/GAZ_00060198">
        <obo:RO_0001025 rdf:resource="http://purl.obolibrary.org/obo/GAZ_00060182"/>
        <obo:IAO_0000115>A lake in the Massif des Cerces.</obo:IAO_0000115>
        <oboInOwl:hasOBONamespace>GAZ</oboInOwl:hasOBONamespace>
        <oboInOwl:id>GAZ:00060198</oboInOwl:id>
        <rdfs:label>Lac Laramon</rdfs:label>
    </owl:NamedIndividual>
    


    <!-- http://purl.obolibrary.org/obo/GAZ_00060199 -->

    <owl:NamedIndividual rdf:about="http://purl.obolibrary.org/obo/GAZ_00060199">
        <obo:RO_0001025 rdf:resource="http://purl.obolibrary.org/obo/GAZ_00060182"/>
        <obo:IAO_0000115>A lake in the Massif des Cerces.</obo:IAO_0000115>
        <oboInOwl:hasOBONamespace>GAZ</oboInOwl:hasOBONamespace>
        <oboInOwl:id>GAZ:00060199</oboInOwl:id>
        <rdfs:label>Lac Long</rdfs:label>
    </owl:NamedIndividual>
    


    <!-- http://purl.obolibrary.org/obo/GAZ_00060200 -->

    <owl:NamedIndividual rdf:about="http://purl.obolibrary.org/obo/GAZ_00060200">
        <obo:RO_0001025 rdf:resource="http://purl.obolibrary.org/obo/GAZ_00060182"/>
        <obo:IAO_0000115>A lake in the Massif des Cerces.</obo:IAO_0000115>
        <oboInOwl:hasOBONamespace>GAZ</oboInOwl:hasOBONamespace>
        <oboInOwl:id>GAZ:00060200</oboInOwl:id>
        <rdfs:label>Lac des Muandes</rdfs:label>
    </owl:NamedIndividual>
    


    <!-- http://purl.obolibrary.org/obo/GAZ_00060201 -->

    <owl:NamedIndividual rdf:about="http://purl.obolibrary.org/obo/GAZ_00060201">
        <obo:RO_0001025 rdf:resource="http://purl.obolibrary.org/obo/GAZ_00060182"/>
        <obo:IAO_0000115>A lake in the Massif des Cerces.</obo:IAO_0000115>
        <oboInOwl:hasOBONamespace>GAZ</oboInOwl:hasOBONamespace>
        <oboInOwl:id>GAZ:00060201</oboInOwl:id>
        <rdfs:label>Lac Noir</rdfs:label>
    </owl:NamedIndividual>
    


    <!-- http://purl.obolibrary.org/obo/GAZ_00060202 -->

    <owl:NamedIndividual rdf:about="http://purl.obolibrary.org/obo/GAZ_00060202">
        <obo:RO_0001025 rdf:resource="http://purl.obolibrary.org/obo/GAZ_00060182"/>
        <obo:IAO_0000115>A glacial lake in the Massif des Cerces.</obo:IAO_0000115>
        <oboInOwl:hasOBONamespace>GAZ</oboInOwl:hasOBONamespace>
        <oboInOwl:id>GAZ:00060202</oboInOwl:id>
        <rdfs:label>Grand lac de l&apos;Oule</rdfs:label>
    </owl:NamedIndividual>
    


    <!-- http://purl.obolibrary.org/obo/GAZ_00060203 -->

    <owl:NamedIndividual rdf:about="http://purl.obolibrary.org/obo/GAZ_00060203">
        <obo:RO_0001025 rdf:resource="http://purl.obolibrary.org/obo/GAZ_00060182"/>
        <obo:IAO_0000115>A lake in the Massif des Cerces.</obo:IAO_0000115>
        <oboInOwl:hasOBONamespace>GAZ</oboInOwl:hasOBONamespace>
        <oboInOwl:id>GAZ:00060203</oboInOwl:id>
        <rdfs:label>Lac de l&apos;Orceyrette</rdfs:label>
    </owl:NamedIndividual>
    


    <!-- http://purl.obolibrary.org/obo/GAZ_00060204 -->

    <owl:NamedIndividual rdf:about="http://purl.obolibrary.org/obo/GAZ_00060204">
        <obo:RO_0001025 rdf:resource="http://purl.obolibrary.org/obo/GAZ_00060182"/>
        <obo:IAO_0000115>A lake in the Massif des Cerces.</obo:IAO_0000115>
        <oboInOwl:hasOBONamespace>GAZ</oboInOwl:hasOBONamespace>
        <oboInOwl:id>GAZ:00060204</oboInOwl:id>
        <rdfs:label>Lac Peyron</rdfs:label>
    </owl:NamedIndividual>
    


    <!-- http://purl.obolibrary.org/obo/GAZ_00060205 -->

    <owl:NamedIndividual rdf:about="http://purl.obolibrary.org/obo/GAZ_00060205">
        <obo:RO_0001025 rdf:resource="http://purl.obolibrary.org/obo/GAZ_00060182"/>
        <obo:IAO_0000115>A lake in the Massif des Cerces.</obo:IAO_0000115>
        <oboInOwl:hasOBONamespace>GAZ</oboInOwl:hasOBONamespace>
        <oboInOwl:id>GAZ:00060205</oboInOwl:id>
        <rdfs:label>Lac de la Ponsonniere</rdfs:label>
    </owl:NamedIndividual>
    


    <!-- http://purl.obolibrary.org/obo/GAZ_00060206 -->

    <owl:NamedIndividual rdf:about="http://purl.obolibrary.org/obo/GAZ_00060206">
        <obo:RO_0001025 rdf:resource="http://purl.obolibrary.org/obo/GAZ_00060182"/>
        <obo:IAO_0000115>A lake in the Massif des Cerces.</obo:IAO_0000115>
        <oboInOwl:hasOBONamespace>GAZ</oboInOwl:hasOBONamespace>
        <oboInOwl:id>GAZ:00060206</oboInOwl:id>
        <rdfs:label>Lac du Serpent</rdfs:label>
    </owl:NamedIndividual>
    


    <!-- http://purl.obolibrary.org/obo/GAZ_00060207 -->

    <owl:NamedIndividual rdf:about="http://purl.obolibrary.org/obo/GAZ_00060207">
        <obo:RO_0001025 rdf:resource="http://purl.obolibrary.org/obo/GAZ_00060182"/>
        <obo:IAO_0000115>A lake in the Massif des Cerces.</obo:IAO_0000115>
        <oboInOwl:hasOBONamespace>GAZ</oboInOwl:hasOBONamespace>
        <oboInOwl:id>GAZ:00060207</oboInOwl:id>
        <rdfs:label>Lac Saraille</rdfs:label>
    </owl:NamedIndividual>
    


    <!-- http://purl.obolibrary.org/obo/GAZ_00060208 -->

    <owl:NamedIndividual rdf:about="http://purl.obolibrary.org/obo/GAZ_00060208">
        <obo:RO_0001025 rdf:resource="http://purl.obolibrary.org/obo/GAZ_00051917"/>
        <obo:RO_0001025 rdf:resource="http://purl.obolibrary.org/obo/GAZ_00060209"/>
        <obo:IAO_0000115>A valley located in the French Hautes-Alpes. Its geographical extension is the basin of river Guil, a tributary of the Durance. Elle est traversee par le Guil et comporte huit communes aujourd&apos;hui regroupees au sein d&apos;une communaute de communes : Arvieux, Abries, Aiguilles, Ceillac, Chateau-Ville-Vieille, Molines-en-Queyras, Ristolas et Saint-Veran.</obo:IAO_0000115>
        <oboInOwl:hasOBONamespace>GAZ</oboInOwl:hasOBONamespace>
        <oboInOwl:id>GAZ:00060208</oboInOwl:id>
        <rdfs:label>Queyras Valley</rdfs:label>
    </owl:NamedIndividual>
    


    <!-- http://purl.obolibrary.org/obo/GAZ_00060209 -->

    <owl:NamedIndividual rdf:about="http://purl.obolibrary.org/obo/GAZ_00060209">
        <obo:RO_0001025 rdf:resource="http://purl.obolibrary.org/obo/GAZ_00008405"/>
        <obo:IAO_0000115>A protected area.</obo:IAO_0000115>
        <oboInOwl:hasOBONamespace>GAZ</oboInOwl:hasOBONamespace>
        <oboInOwl:id>GAZ:00060209</oboInOwl:id>
        <rdfs:label>Parc naturel regional du Queyras</rdfs:label>
    </owl:NamedIndividual>
    


    <!-- http://purl.obolibrary.org/obo/GAZ_00060210 -->

    <owl:NamedIndividual rdf:about="http://purl.obolibrary.org/obo/GAZ_00060210">
        <obo:RO_0001025 rdf:resource="http://purl.obolibrary.org/obo/GAZ_00060218"/>
        <obo:IAO_0000115>Un lac se trouve a 2215 m, en dessous du lac Saint-Anne.</obo:IAO_0000115>
        <oboInOwl:hasOBONamespace>GAZ</oboInOwl:hasOBONamespace>
        <oboInOwl:id>GAZ:00060210</oboInOwl:id>
        <rdfs:label>Lac Miroir</rdfs:label>
    </owl:NamedIndividual>
    


    <!-- http://purl.obolibrary.org/obo/GAZ_00060211 -->

    <owl:NamedIndividual rdf:about="http://purl.obolibrary.org/obo/GAZ_00060211">
        <obo:RO_0001025 rdf:resource="http://purl.obolibrary.org/obo/GAZ_00060208"/>
        <obo:RO_0001025 rdf:resource="http://purl.obolibrary.org/obo/GAZ_00060218"/>
        <obo:IAO_0000115>Un lac situe au sud du parc regional du Queyras, dans les Hautes-Alpes, a 2414 m d&apos;altitude, au pied du Pic Nord de la Font Sancte.</obo:IAO_0000115>
        <oboInOwl:hasOBONamespace>GAZ</oboInOwl:hasOBONamespace>
        <oboInOwl:id>GAZ:00060211</oboInOwl:id>
        <rdfs:label>Lac Saint-Anne</rdfs:label>
    </owl:NamedIndividual>
    


    <!-- http://purl.obolibrary.org/obo/GAZ_00060212 -->

    <owl:NamedIndividual rdf:about="http://purl.obolibrary.org/obo/GAZ_00060212">
        <obo:RO_0001025 rdf:resource="http://purl.obolibrary.org/obo/GAZ_00060208"/>
        <obo:IAO_0000115>Lakes in the Queyras Valley.</obo:IAO_0000115>
        <oboInOwl:hasOBONamespace>GAZ</oboInOwl:hasOBONamespace>
        <oboInOwl:id>GAZ:00060212</oboInOwl:id>
        <rdfs:label>Les Lacs du Malrif</rdfs:label>
    </owl:NamedIndividual>
    


    <!-- http://purl.obolibrary.org/obo/GAZ_00060213 -->

    <owl:NamedIndividual rdf:about="http://purl.obolibrary.org/obo/GAZ_00060213">
        <obo:RO_0001025 rdf:resource="http://purl.obolibrary.org/obo/GAZ_00060208"/>
        <obo:IAO_0000115>A lake in the Queyras Valley.</obo:IAO_0000115>
        <oboInOwl:hasOBONamespace>GAZ</oboInOwl:hasOBONamespace>
        <oboInOwl:id>GAZ:00060213</oboInOwl:id>
        <rdfs:label>Lac de Souliers</rdfs:label>
    </owl:NamedIndividual>
    


    <!-- http://purl.obolibrary.org/obo/GAZ_00060214 -->

    <owl:NamedIndividual rdf:about="http://purl.obolibrary.org/obo/GAZ_00060214">
        <obo:RO_0001025 rdf:resource="http://purl.obolibrary.org/obo/GAZ_00060208"/>
        <obo:IAO_0000115>A lake in the Queyras Valley.</obo:IAO_0000115>
        <oboInOwl:hasOBONamespace>GAZ</oboInOwl:hasOBONamespace>
        <oboInOwl:id>GAZ:00060214</oboInOwl:id>
        <rdfs:label>Le Lac Foreant</rdfs:label>
    </owl:NamedIndividual>
    


    <!-- http://purl.obolibrary.org/obo/GAZ_00060216 -->

    <owl:NamedIndividual rdf:about="http://purl.obolibrary.org/obo/GAZ_00060216">
        <obo:RO_0001025 rdf:resource="http://purl.obolibrary.org/obo/GAZ_00060208"/>
        <obo:IAO_0000115>A lake in the Queyras Valley.</obo:IAO_0000115>
        <oboInOwl:hasOBONamespace>GAZ</oboInOwl:hasOBONamespace>
        <oboInOwl:id>GAZ:00060216</oboInOwl:id>
        <rdfs:label>Lac Escur</rdfs:label>
    </owl:NamedIndividual>
    


    <!-- http://purl.obolibrary.org/obo/GAZ_00060217 -->

    <owl:NamedIndividual rdf:about="http://purl.obolibrary.org/obo/GAZ_00060217">
        <obo:RO_0001025 rdf:resource="http://purl.obolibrary.org/obo/GAZ_00060208"/>
        <obo:IAO_0000115>A lake in the Queyras Valley.</obo:IAO_0000115>
        <oboInOwl:hasOBONamespace>GAZ</oboInOwl:hasOBONamespace>
        <oboInOwl:id>GAZ:00060217</oboInOwl:id>
        <rdfs:label>Lac de l&apos;Ascension</rdfs:label>
    </owl:NamedIndividual>
    


    <!-- http://purl.obolibrary.org/obo/GAZ_00060218 -->

    <owl:NamedIndividual rdf:about="http://purl.obolibrary.org/obo/GAZ_00060218">
        <obo:RO_0001025 rdf:resource="http://purl.obolibrary.org/obo/GAZ_00060208"/>
        <obo:IAO_0000115>Lakes in the Queyras Valley.</obo:IAO_0000115>
        <oboInOwl:hasOBONamespace>GAZ</oboInOwl:hasOBONamespace>
        <oboInOwl:id>GAZ:00060218</oboInOwl:id>
        <rdfs:label>Lacs de Ceillac</rdfs:label>
    </owl:NamedIndividual>
    


    <!-- http://purl.obolibrary.org/obo/GAZ_00060219 -->

    <owl:NamedIndividual rdf:about="http://purl.obolibrary.org/obo/GAZ_00060219">
        <obo:RO_0001025 rdf:resource="http://purl.obolibrary.org/obo/GAZ_00060208"/>
        <obo:IAO_0000115>A lake in the Queyras Valley.</obo:IAO_0000115>
        <oboInOwl:hasOBONamespace>GAZ</oboInOwl:hasOBONamespace>
        <oboInOwl:id>GAZ:00060219</oboInOwl:id>
        <rdfs:label>Lac de la Blanche</rdfs:label>
    </owl:NamedIndividual>
    


    <!-- http://purl.obolibrary.org/obo/GAZ_00060220 -->

    <owl:NamedIndividual rdf:about="http://purl.obolibrary.org/obo/GAZ_00060220">
        <obo:RO_0001025 rdf:resource="http://purl.obolibrary.org/obo/GAZ_00060208"/>
        <obo:IAO_0000115>Lakes in the Queyras Valley.</obo:IAO_0000115>
        <oboInOwl:hasOBONamespace>GAZ</oboInOwl:hasOBONamespace>
        <oboInOwl:id>GAZ:00060220</oboInOwl:id>
        <rdfs:label>Lacs Blanchets</rdfs:label>
    </owl:NamedIndividual>
    


    <!-- http://purl.obolibrary.org/obo/GAZ_00060221 -->

    <owl:NamedIndividual rdf:about="http://purl.obolibrary.org/obo/GAZ_00060221">
        <obo:RO_0001025 rdf:resource="http://purl.obolibrary.org/obo/GAZ_00060208"/>
        <obo:IAO_0000115>A lake in the Queyras Valley.</obo:IAO_0000115>
        <oboInOwl:hasOBONamespace>GAZ</oboInOwl:hasOBONamespace>
        <oboInOwl:id>GAZ:00060221</oboInOwl:id>
        <rdfs:label>Lac d&apos;Asti</rdfs:label>
    </owl:NamedIndividual>
    


    <!-- http://purl.obolibrary.org/obo/GAZ_00060222 -->

    <owl:NamedIndividual rdf:about="http://purl.obolibrary.org/obo/GAZ_00060222">
        <obo:RO_0001025 rdf:resource="http://purl.obolibrary.org/obo/GAZ_00060208"/>
        <obo:IAO_0000115>A lake in the Queyras Valley.</obo:IAO_0000115>
        <oboInOwl:hasOBONamespace>GAZ</oboInOwl:hasOBONamespace>
        <oboInOwl:id>GAZ:00060222</oboInOwl:id>
        <rdfs:label>Lac Clausis</rdfs:label>
    </owl:NamedIndividual>
    


    <!-- http://purl.obolibrary.org/obo/GAZ_00060223 -->

    <owl:NamedIndividual rdf:about="http://purl.obolibrary.org/obo/GAZ_00060223">
        <obo:RO_0001025 rdf:resource="http://purl.obolibrary.org/obo/GAZ_00060208"/>
        <obo:IAO_0000115>A lake in the Queyras Valley.</obo:IAO_0000115>
        <oboInOwl:hasOBONamespace>GAZ</oboInOwl:hasOBONamespace>
        <oboInOwl:id>GAZ:00060223</oboInOwl:id>
        <rdfs:label>Lac Chalanties</rdfs:label>
    </owl:NamedIndividual>
    


    <!-- http://purl.obolibrary.org/obo/GAZ_00060224 -->

    <owl:NamedIndividual rdf:about="http://purl.obolibrary.org/obo/GAZ_00060224">
        <obo:RO_0001025 rdf:resource="http://purl.obolibrary.org/obo/GAZ_00060218"/>
        <obo:IAO_0000115>A lake in the Queyras Valley.</obo:IAO_0000115>
        <oboInOwl:hasOBONamespace>GAZ</oboInOwl:hasOBONamespace>
        <oboInOwl:id>GAZ:00060224</oboInOwl:id>
        <rdfs:label>Lac des Rouites</rdfs:label>
    </owl:NamedIndividual>
    


    <!-- http://purl.obolibrary.org/obo/GAZ_00060229 -->

    <owl:NamedIndividual rdf:about="http://purl.obolibrary.org/obo/GAZ_00060229">
        <obo:RO_0001025 rdf:resource="http://purl.obolibrary.org/obo/GAZ_00060208"/>
        <obo:IAO_0000115>Un lac alpin, situe sur la commune de Cervieres dans les Hautes-Alpes, a de 2446 m.</obo:IAO_0000115>
        <oboInOwl:hasOBONamespace>GAZ</oboInOwl:hasOBONamespace>
        <oboInOwl:id>GAZ:00060229</oboInOwl:id>
        <rdfs:label>Lac des Cordes</rdfs:label>
    </owl:NamedIndividual>
    


    <!-- http://purl.obolibrary.org/obo/GAZ_00060230 -->

    <owl:NamedIndividual rdf:about="http://purl.obolibrary.org/obo/GAZ_00060230">
        <obo:RO_0001025 rdf:resource="http://purl.obolibrary.org/obo/GAZ_00060208"/>
        <obo:IAO_0000115>A lake in the Queyras Valley.</obo:IAO_0000115>
        <oboInOwl:hasOBONamespace>GAZ</oboInOwl:hasOBONamespace>
        <oboInOwl:id>GAZ:00060230</oboInOwl:id>
        <rdfs:label>Lac Lacroix</rdfs:label>
    </owl:NamedIndividual>
    


    <!-- http://purl.obolibrary.org/obo/GAZ_00060231 -->

    <owl:NamedIndividual rdf:about="http://purl.obolibrary.org/obo/GAZ_00060231">
        <obo:RO_0001025 rdf:resource="http://purl.obolibrary.org/obo/GAZ_00060208"/>
        <obo:IAO_0000115>A lake in the Queyras Valley.</obo:IAO_0000115>
        <oboInOwl:hasOBONamespace>GAZ</oboInOwl:hasOBONamespace>
        <oboInOwl:id>GAZ:00060231</oboInOwl:id>
        <rdfs:label>Lac Lestio</rdfs:label>
    </owl:NamedIndividual>
    


    <!-- http://purl.obolibrary.org/obo/GAZ_00060232 -->

    <owl:NamedIndividual rdf:about="http://purl.obolibrary.org/obo/GAZ_00060232">
        <obo:RO_0001025 rdf:resource="http://purl.obolibrary.org/obo/GAZ_00060208"/>
    </owl:NamedIndividual>
    


    <!-- http://purl.obolibrary.org/obo/GAZ_00060233 -->

    <owl:NamedIndividual rdf:about="http://purl.obolibrary.org/obo/GAZ_00060233">
        <obo:RO_0001025 rdf:resource="http://purl.obolibrary.org/obo/GAZ_00060208"/>
    </owl:NamedIndividual>
    


    <!-- http://purl.obolibrary.org/obo/GAZ_00060234 -->

    <owl:NamedIndividual rdf:about="http://purl.obolibrary.org/obo/GAZ_00060234">
        <obo:RO_0001025 rdf:resource="http://purl.obolibrary.org/obo/GAZ_00060208"/>
        <obo:IAO_0000115>A lake in the Queyras Valley.</obo:IAO_0000115>
        <oboInOwl:hasOBONamespace>GAZ</oboInOwl:hasOBONamespace>
        <oboInOwl:id>GAZ:00060234</oboInOwl:id>
        <rdfs:label>Lac de l&apos;Eychassier</rdfs:label>
    </owl:NamedIndividual>
    


    <!-- http://purl.obolibrary.org/obo/GAZ_00060237 -->

    <owl:NamedIndividual rdf:about="http://purl.obolibrary.org/obo/GAZ_00060237">
        <obo:RO_0001025 rdf:resource="http://purl.obolibrary.org/obo/GAZ_00060208"/>
        <obo:IAO_0000115>A lake in the Queyras Valley.</obo:IAO_0000115>
        <oboInOwl:hasOBONamespace>GAZ</oboInOwl:hasOBONamespace>
        <oboInOwl:id>GAZ:00060237</oboInOwl:id>
        <rdfs:label>Lac Jean Rostand</rdfs:label>
    </owl:NamedIndividual>
    


    <!-- http://purl.obolibrary.org/obo/GAZ_00060240 -->

    <owl:NamedIndividual rdf:about="http://purl.obolibrary.org/obo/GAZ_00060240">
        <obo:RO_0001025 rdf:resource="http://purl.obolibrary.org/obo/GAZ_00060208"/>
    </owl:NamedIndividual>
    


    <!-- http://purl.obolibrary.org/obo/GAZ_00060241 -->

    <owl:NamedIndividual rdf:about="http://purl.obolibrary.org/obo/GAZ_00060241">
        <obo:RO_0001025 rdf:resource="http://purl.obolibrary.org/obo/GAZ_00060208"/>
        <obo:IAO_0000115>A lake in the Queyras Valley.</obo:IAO_0000115>
        <oboInOwl:hasOBONamespace>GAZ</oboInOwl:hasOBONamespace>
        <oboInOwl:id>GAZ:00060241</oboInOwl:id>
        <rdfs:label>Grand lac du Lauzet</rdfs:label>
    </owl:NamedIndividual>
    


    <!-- http://purl.obolibrary.org/obo/GAZ_00060242 -->

    <owl:NamedIndividual rdf:about="http://purl.obolibrary.org/obo/GAZ_00060242">
        <obo:RO_0001025 rdf:resource="http://purl.obolibrary.org/obo/GAZ_00060208"/>
        <obo:IAO_0000115>A lake in the Queyras Valley.</obo:IAO_0000115>
        <oboInOwl:hasOBONamespace>GAZ</oboInOwl:hasOBONamespace>
        <oboInOwl:id>GAZ:00060242</oboInOwl:id>
        <rdfs:label>Lac Lauzon</rdfs:label>
    </owl:NamedIndividual>
    


    <!-- http://purl.obolibrary.org/obo/GAZ_00060243 -->

    <owl:NamedIndividual rdf:about="http://purl.obolibrary.org/obo/GAZ_00060243">
        <obo:RO_0001025 rdf:resource="http://purl.obolibrary.org/obo/GAZ_00060208"/>
        <oboInOwl:hasOBONamespace>GAZ</oboInOwl:hasOBONamespace>
        <oboInOwl:id>GAZ:00060243</oboInOwl:id>
        <rdfs:label>Lac Neal</rdfs:label>
    </owl:NamedIndividual>
    


    <!-- http://purl.obolibrary.org/obo/GAZ_00060244 -->

    <owl:NamedIndividual rdf:about="http://purl.obolibrary.org/obo/GAZ_00060244">
        <obo:RO_0001025 rdf:resource="http://purl.obolibrary.org/obo/GAZ_00060208"/>
        <obo:IAO_0000115>A lake in the Queyras Valley.</obo:IAO_0000115>
        <oboInOwl:hasOBONamespace>GAZ</oboInOwl:hasOBONamespace>
        <oboInOwl:id>GAZ:00060244</oboInOwl:id>
        <rdfs:label>Lac Lauzon de Furfande</rdfs:label>
    </owl:NamedIndividual>
    


    <!-- http://purl.obolibrary.org/obo/GAZ_00060245 -->

    <owl:NamedIndividual rdf:about="http://purl.obolibrary.org/obo/GAZ_00060245">
        <obo:RO_0001025 rdf:resource="http://purl.obolibrary.org/obo/GAZ_00060208"/>
        <obo:IAO_0000115>A lake in the Queyras Valley.</obo:IAO_0000115>
        <oboInOwl:hasOBONamespace>GAZ</oboInOwl:hasOBONamespace>
        <oboInOwl:id>GAZ:00060245</oboInOwl:id>
        <rdfs:label>Lac moyen du Lauzet</rdfs:label>
    </owl:NamedIndividual>
    


    <!-- http://purl.obolibrary.org/obo/GAZ_00060249 -->

    <owl:NamedIndividual rdf:about="http://purl.obolibrary.org/obo/GAZ_00060249">
        <obo:RO_0001025 rdf:resource="http://purl.obolibrary.org/obo/GAZ_00060208"/>
        <obo:IAO_0000115>A lake in the Queyras Valley.</obo:IAO_0000115>
        <oboInOwl:hasOBONamespace>GAZ</oboInOwl:hasOBONamespace>
        <oboInOwl:id>GAZ:00060249</oboInOwl:id>
        <rdfs:label>Lac ouest de Rasis</rdfs:label>
    </owl:NamedIndividual>
    


    <!-- http://purl.obolibrary.org/obo/GAZ_00060250 -->

    <owl:NamedIndividual rdf:about="http://purl.obolibrary.org/obo/GAZ_00060250">
        <obo:RO_0001025 rdf:resource="http://purl.obolibrary.org/obo/GAZ_00060208"/>
        <obo:IAO_0000115>A lake in the Queyras Valley.</obo:IAO_0000115>
        <oboInOwl:hasOBONamespace>GAZ</oboInOwl:hasOBONamespace>
        <oboInOwl:id>GAZ:00060250</oboInOwl:id>
        <rdfs:label>Lac Petit-Laus</rdfs:label>
    </owl:NamedIndividual>
    


    <!-- http://purl.obolibrary.org/obo/GAZ_00060251 -->

    <owl:NamedIndividual rdf:about="http://purl.obolibrary.org/obo/GAZ_00060251">
        <obo:RO_0001025 rdf:resource="http://purl.obolibrary.org/obo/GAZ_00060208"/>
        <obo:IAO_0000115>A lake in the Queyras Valley.</obo:IAO_0000115>
        <oboInOwl:hasOBONamespace>GAZ</oboInOwl:hasOBONamespace>
        <oboInOwl:id>GAZ:00060251</oboInOwl:id>
        <rdfs:label>Lac de Rasis</rdfs:label>
    </owl:NamedIndividual>
    


    <!-- http://purl.obolibrary.org/obo/GAZ_00060252 -->

    <owl:NamedIndividual rdf:about="http://purl.obolibrary.org/obo/GAZ_00060252">
        <obo:RO_0001025 rdf:resource="http://purl.obolibrary.org/obo/GAZ_00060208"/>
        <obo:IAO_0000115>A lake in the Queyras Valley.</obo:IAO_0000115>
        <oboInOwl:hasOBONamespace>GAZ</oboInOwl:hasOBONamespace>
        <oboInOwl:id>GAZ:00060252</oboInOwl:id>
        <rdfs:label>Lac Haut-Neal</rdfs:label>
    </owl:NamedIndividual>
    


    <!-- http://purl.obolibrary.org/obo/GAZ_00060253 -->

    <owl:NamedIndividual rdf:about="http://purl.obolibrary.org/obo/GAZ_00060253">
        <obo:RO_0001025 rdf:resource="http://purl.obolibrary.org/obo/GAZ_00060208"/>
        <obo:IAO_0000115>A lake in the Queyras Valley.</obo:IAO_0000115>
        <oboInOwl:hasOBONamespace>GAZ</oboInOwl:hasOBONamespace>
        <oboInOwl:id>GAZ:00060253</oboInOwl:id>
        <rdfs:label>Lac des Neuf-couleurs</rdfs:label>
    </owl:NamedIndividual>
    


    <!-- http://purl.obolibrary.org/obo/GAZ_00060254 -->

    <owl:NamedIndividual rdf:about="http://purl.obolibrary.org/obo/GAZ_00060254">
        <obo:RO_0001025 rdf:resource="http://purl.obolibrary.org/obo/GAZ_00060208"/>
        <obo:IAO_0000115>A lake in the Queyras Valley.</obo:IAO_0000115>
        <oboInOwl:hasOBONamespace>GAZ</oboInOwl:hasOBONamespace>
        <oboInOwl:id>GAZ:00060254</oboInOwl:id>
        <rdfs:label>Lago Verde</rdfs:label>
    </owl:NamedIndividual>
    


    <!-- http://purl.obolibrary.org/obo/GAZ_00060255 -->

    <owl:NamedIndividual rdf:about="http://purl.obolibrary.org/obo/GAZ_00060255">
        <obo:RO_0001025 rdf:resource="http://purl.obolibrary.org/obo/GAZ_00009675"/>
        <obo:IAO_0000115>A national park located in the south-eastern part of France and consists in a mountainous region of the Dauphine Alps, south of Grenoble and north of Gap, shared between the departements of Isere and Hautes-Alpes. Its borders mostly correspond to these of the Massif des Ecrins, delimited by the main valleys of rivers Drac, Romanche and Durance (with its Guisane dependancy).</obo:IAO_0000115>
        <oboInOwl:hasOBONamespace>GAZ</oboInOwl:hasOBONamespace>
        <oboInOwl:id>GAZ:00060255</oboInOwl:id>
        <rdfs:label>Parc national des Ecrins</rdfs:label>
    </owl:NamedIndividual>
    


    <!-- http://purl.obolibrary.org/obo/GAZ_00060256 -->

    <owl:NamedIndividual rdf:about="http://purl.obolibrary.org/obo/GAZ_00060256">
        <obo:RO_0001025 rdf:resource="http://purl.obolibrary.org/obo/GAZ_00060255"/>
        <obo:IAO_0000115>A mountain massif that form the core of the Parc national des Ecrins in France.</obo:IAO_0000115>
        <oboInOwl:hasOBONamespace>GAZ</oboInOwl:hasOBONamespace>
        <oboInOwl:id>GAZ:00060256</oboInOwl:id>
        <rdfs:label>Massif des Ecrins</rdfs:label>
    </owl:NamedIndividual>
    


    <!-- http://purl.obolibrary.org/obo/GAZ_00060257 -->

    <owl:NamedIndividual rdf:about="http://purl.obolibrary.org/obo/GAZ_00060257">
        <obo:RO_0001025 rdf:resource="http://purl.obolibrary.org/obo/GAZ_00060256"/>
        <obo:IAO_0000115>A lake in the Hautes-Alpes.</obo:IAO_0000115>
        <oboInOwl:hasOBONamespace>GAZ</oboInOwl:hasOBONamespace>
        <oboInOwl:id>GAZ:00060257</oboInOwl:id>
        <rdfs:label>Lac de Combeynot</rdfs:label>
    </owl:NamedIndividual>
    


    <!-- http://purl.obolibrary.org/obo/GAZ_00060261 -->

    <owl:NamedIndividual rdf:about="http://purl.obolibrary.org/obo/GAZ_00060261">
        <obo:RO_0001025 rdf:resource="http://purl.obolibrary.org/obo/GAZ_00060256"/>
        <obo:IAO_0000115>A lake in the Massif des Ecrins, Hautes-Alpes.</obo:IAO_0000115>
        <oboInOwl:hasOBONamespace>GAZ</oboInOwl:hasOBONamespace>
        <oboInOwl:id>GAZ:00060261</oboInOwl:id>
        <rdfs:label>Lac de Dormillouse</rdfs:label>
    </owl:NamedIndividual>
    


    <!-- http://purl.obolibrary.org/obo/GAZ_00060262 -->

    <owl:NamedIndividual rdf:about="http://purl.obolibrary.org/obo/GAZ_00060262">
        <obo:RO_0001025 rdf:resource="http://purl.obolibrary.org/obo/GAZ_00060256"/>
        <obo:IAO_0000115>Un lac situe en zone central du parc national des Ecrins par Vallouise et la commune de Pelvoux a 2514 m.</obo:IAO_0000115>
        <oboInOwl:hasOBONamespace>GAZ</oboInOwl:hasOBONamespace>
        <oboInOwl:id>GAZ:00060262</oboInOwl:id>
        <rdfs:label>Lac de l&apos;Eychauda</rdfs:label>
    </owl:NamedIndividual>
    


    <!-- http://purl.obolibrary.org/obo/GAZ_00060265 -->

    <owl:NamedIndividual rdf:about="http://purl.obolibrary.org/obo/GAZ_00060265">
        <obo:RO_0001025 rdf:resource="http://purl.obolibrary.org/obo/GAZ_00060256"/>
        <obo:IAO_0000115>A lake in the Massif des Ecrins, Hautes-Alpes.</obo:IAO_0000115>
        <oboInOwl:hasOBONamespace>GAZ</oboInOwl:hasOBONamespace>
        <oboInOwl:id>GAZ:00060265</oboInOwl:id>
        <rdfs:label>Lac Faravel</rdfs:label>
    </owl:NamedIndividual>
    


    <!-- http://purl.obolibrary.org/obo/GAZ_00060266 -->

    <owl:NamedIndividual rdf:about="http://purl.obolibrary.org/obo/GAZ_00060266">
        <obo:RO_0001025 rdf:resource="http://purl.obolibrary.org/obo/GAZ_00060256"/>
        <obo:IAO_0000115>Lakes in the Massif des Ecrins, Hautes-Alpes.</obo:IAO_0000115>
        <oboInOwl:hasOBONamespace>GAZ</oboInOwl:hasOBONamespace>
        <oboInOwl:id>GAZ:00060266</oboInOwl:id>
        <rdfs:label>Lacs Jumeaux</rdfs:label>
    </owl:NamedIndividual>
    


    <!-- http://purl.obolibrary.org/obo/GAZ_00060267 -->

    <owl:NamedIndividual rdf:about="http://purl.obolibrary.org/obo/GAZ_00060267">
        <obo:RO_0001025 rdf:resource="http://purl.obolibrary.org/obo/GAZ_00060256"/>
        <obo:IAO_0000115>A lake in the Massif des Ecrins, Hautes-Alpes.</obo:IAO_0000115>
        <oboInOwl:hasOBONamespace>GAZ</oboInOwl:hasOBONamespace>
        <oboInOwl:id>GAZ:00060267</oboInOwl:id>
        <rdfs:label>Lac du Lauzon</rdfs:label>
    </owl:NamedIndividual>
    


    <!-- http://purl.obolibrary.org/obo/GAZ_00060268 -->

    <owl:NamedIndividual rdf:about="http://purl.obolibrary.org/obo/GAZ_00060268">
        <obo:RO_0001025 rdf:resource="http://purl.obolibrary.org/obo/GAZ_00060256"/>
        <obo:IAO_0000115>A lake in the Massif des Ecrins, Hautes-Alpes.</obo:IAO_0000115>
        <oboInOwl:hasOBONamespace>GAZ</oboInOwl:hasOBONamespace>
        <oboInOwl:id>GAZ:00060268</oboInOwl:id>
        <rdfs:label>Lac Long</rdfs:label>
    </owl:NamedIndividual>
    


    <!-- http://purl.obolibrary.org/obo/GAZ_00060269 -->

    <owl:NamedIndividual rdf:about="http://purl.obolibrary.org/obo/GAZ_00060269">
        <obo:RO_0001025 rdf:resource="http://purl.obolibrary.org/obo/GAZ_00060256"/>
        <obo:IAO_0000115>A lake in the Massif des Ecrins, Hautes-Alpes.</obo:IAO_0000115>
        <oboInOwl:hasOBONamespace>GAZ</oboInOwl:hasOBONamespace>
        <oboInOwl:id>GAZ:00060269</oboInOwl:id>
        <rdfs:label>Lac Palluel</rdfs:label>
    </owl:NamedIndividual>
    


    <!-- http://purl.obolibrary.org/obo/GAZ_00060270 -->

    <owl:NamedIndividual rdf:about="http://purl.obolibrary.org/obo/GAZ_00060270">
        <obo:RO_0001025 rdf:resource="http://purl.obolibrary.org/obo/GAZ_00060256"/>
        <obo:IAO_0000115>A lake in the Massif des Ecrins, Hautes-Alpes.</obo:IAO_0000115>
        <oboInOwl:hasOBONamespace>GAZ</oboInOwl:hasOBONamespace>
        <oboInOwl:id>GAZ:00060270</oboInOwl:id>
        <rdfs:label>Lac de Puy Vachier</rdfs:label>
    </owl:NamedIndividual>
    


    <!-- http://purl.obolibrary.org/obo/GAZ_00060271 -->

    <owl:NamedIndividual rdf:about="http://purl.obolibrary.org/obo/GAZ_00060271">
        <obo:RO_0001025 rdf:resource="http://purl.obolibrary.org/obo/GAZ_00060256"/>
        <obo:IAO_0000115>A lake in the Massif des Ecrins, Hautes-Alpes.</obo:IAO_0000115>
        <oboInOwl:hasOBONamespace>GAZ</oboInOwl:hasOBONamespace>
        <oboInOwl:id>GAZ:00060271</oboInOwl:id>
        <rdfs:label>Lac des Pisses</rdfs:label>
    </owl:NamedIndividual>
    


    <!-- http://purl.obolibrary.org/obo/GAZ_00060272 -->

    <owl:NamedIndividual rdf:about="http://purl.obolibrary.org/obo/GAZ_00060272">
        <obo:RO_0001025 rdf:resource="http://purl.obolibrary.org/obo/GAZ_00060256"/>
        <obo:IAO_0000115>Un lac situe sur la commune d&apos;Orcieres-Merlette (Hautes-Alpes) dans le Champsaur (massif des Ecrins), a une altitude de 2390 m.</obo:IAO_0000115>
        <oboInOwl:hasOBONamespace>GAZ</oboInOwl:hasOBONamespace>
        <oboInOwl:id>GAZ:00060272</oboInOwl:id>
        <rdfs:label>Lac des Sirenes</rdfs:label>
    </owl:NamedIndividual>
    


    <!-- http://purl.obolibrary.org/obo/GAZ_00060273 -->

    <owl:NamedIndividual rdf:about="http://purl.obolibrary.org/obo/GAZ_00060273">
        <obo:RO_0001025 rdf:resource="http://purl.obolibrary.org/obo/GAZ_00060256"/>
        <obo:IAO_0000115>A lake in the Massif des Ecrins, Hautes-Alpes.</obo:IAO_0000115>
        <oboInOwl:hasOBONamespace>GAZ</oboInOwl:hasOBONamespace>
        <oboInOwl:id>GAZ:00060273</oboInOwl:id>
        <rdfs:label>Lac Profond</rdfs:label>
    </owl:NamedIndividual>
    


    <!-- http://purl.obolibrary.org/obo/GAZ_00060288 -->

    <owl:NamedIndividual rdf:about="http://purl.obolibrary.org/obo/GAZ_00060288">
        <obo:RO_0001025 rdf:resource="http://purl.obolibrary.org/obo/GAZ_00006787"/>
        <obo:IAO_0000115>Part of the Massif du Luberon.</obo:IAO_0000115>
        <oboInOwl:hasOBONamespace>GAZ</oboInOwl:hasOBONamespace>
        <oboInOwl:id>GAZ:00060288</oboInOwl:id>
        <rdfs:label>Luberon oriental</rdfs:label>
    </owl:NamedIndividual>
    


    <!-- http://purl.obolibrary.org/obo/GAZ_00060289 -->

    <owl:NamedIndividual rdf:about="http://purl.obolibrary.org/obo/GAZ_00060289">
        <obo:RO_0001025 rdf:resource="http://purl.obolibrary.org/obo/GAZ_00006787"/>
        <obo:IAO_0000115>Part of the Massif du Luberon.</obo:IAO_0000115>
        <oboInOwl:hasOBONamespace>GAZ</oboInOwl:hasOBONamespace>
        <oboInOwl:id>GAZ:00060289</oboInOwl:id>
        <rdfs:label>Grand Luberon</rdfs:label>
    </owl:NamedIndividual>
    


    <!-- http://purl.obolibrary.org/obo/GAZ_00060290 -->

    <owl:NamedIndividual rdf:about="http://purl.obolibrary.org/obo/GAZ_00060290">
        <obo:RO_0001025 rdf:resource="http://purl.obolibrary.org/obo/GAZ_00006787"/>
        <obo:IAO_0000115>Part of the Massif du Luberon.</obo:IAO_0000115>
        <oboInOwl:hasOBONamespace>GAZ</oboInOwl:hasOBONamespace>
        <oboInOwl:id>GAZ:00060290</oboInOwl:id>
        <rdfs:label>Petit Luberon</rdfs:label>
    </owl:NamedIndividual>
    


    <!-- http://purl.obolibrary.org/obo/GAZ_00060291 -->

    <owl:NamedIndividual rdf:about="http://purl.obolibrary.org/obo/GAZ_00060291">
        <obo:RO_0001025 rdf:resource="http://purl.obolibrary.org/obo/GAZ_00051917"/>
        <obo:RO_0001025 rdf:resource="http://purl.obolibrary.org/obo/GAZ_00060318"/>
        <obo:IAO_0000115>A glacial valley in the Alpes de Haute-Provence departement, in the French Alps.</obo:IAO_0000115>
        <oboInOwl:hasOBONamespace>GAZ</oboInOwl:hasOBONamespace>
        <oboInOwl:id>GAZ:00060291</oboInOwl:id>
        <rdfs:label>Ubaye Valley</rdfs:label>
    </owl:NamedIndividual>
    


    <!-- http://purl.obolibrary.org/obo/GAZ_00060292 -->

    <owl:NamedIndividual rdf:about="http://purl.obolibrary.org/obo/GAZ_00060292">
        <obo:RO_0001025 rdf:resource="http://purl.obolibrary.org/obo/GAZ_00008405"/>
        <obo:IAO_0000115>Un massif des Alpes internes.</obo:IAO_0000115>
        <oboInOwl:hasOBONamespace>GAZ</oboInOwl:hasOBONamespace>
        <oboInOwl:id>GAZ:00060292</oboInOwl:id>
        <rdfs:label>Massif de Chambeyron</rdfs:label>
    </owl:NamedIndividual>
    


    <!-- http://purl.obolibrary.org/obo/GAZ_00060293 -->

    <owl:NamedIndividual rdf:about="http://purl.obolibrary.org/obo/GAZ_00060293">
        <obo:RO_0001025 rdf:resource="http://purl.obolibrary.org/obo/GAZ_00060291"/>
        <obo:IAO_0000115>A lake in the Ubaye Valley.</obo:IAO_0000115>
        <oboInOwl:hasOBONamespace>GAZ</oboInOwl:hasOBONamespace>
        <oboInOwl:id>GAZ:00060293</oboInOwl:id>
        <rdfs:label>Lac de la Petite Cayolle</rdfs:label>
    </owl:NamedIndividual>
    


    <!-- http://purl.obolibrary.org/obo/GAZ_00060294 -->

    <owl:NamedIndividual rdf:about="http://purl.obolibrary.org/obo/GAZ_00060294">
        <obo:RO_0001025 rdf:resource="http://purl.obolibrary.org/obo/GAZ_00060291"/>
        <obo:IAO_0000115>A lake in the Ubaye Valley.</obo:IAO_0000115>
        <oboInOwl:hasOBONamespace>GAZ</oboInOwl:hasOBONamespace>
        <oboInOwl:id>GAZ:00060294</oboInOwl:id>
        <rdfs:label>Lac des Hommes</rdfs:label>
    </owl:NamedIndividual>
    


    <!-- http://purl.obolibrary.org/obo/GAZ_00060295 -->

    <owl:NamedIndividual rdf:about="http://purl.obolibrary.org/obo/GAZ_00060295">
        <obo:RO_0001025 rdf:resource="http://purl.obolibrary.org/obo/GAZ_00060291"/>
        <obo:IAO_0000115>A lake in the Ubaye Valley.</obo:IAO_0000115>
        <oboInOwl:hasOBONamespace>GAZ</oboInOwl:hasOBONamespace>
        <oboInOwl:id>GAZ:00060295</oboInOwl:id>
        <rdfs:label>Lac de l&apos;Oronaye</rdfs:label>
    </owl:NamedIndividual>
    


    <!-- http://purl.obolibrary.org/obo/GAZ_00060296 -->

    <owl:NamedIndividual rdf:about="http://purl.obolibrary.org/obo/GAZ_00060296">
        <obo:RO_0001025 rdf:resource="http://purl.obolibrary.org/obo/GAZ_00060299"/>
        <obo:IAO_0000115>The smaller of the two lower Lacs de Marinet.</obo:IAO_0000115>
        <oboInOwl:hasOBONamespace>GAZ</oboInOwl:hasOBONamespace>
        <oboInOwl:id>GAZ:00060296</oboInOwl:id>
        <rdfs:label>Lac-petit du Marinet</rdfs:label>
    </owl:NamedIndividual>
    


    <!-- http://purl.obolibrary.org/obo/GAZ_00060298 -->

    <owl:NamedIndividual rdf:about="http://purl.obolibrary.org/obo/GAZ_00060298">
        <obo:RO_0001025 rdf:resource="http://purl.obolibrary.org/obo/GAZ_00060318"/>
        <obo:IAO_0000115>A glacial lake, in the Department of Alpes-de-Haute-Provence.</obo:IAO_0000115>
        <oboInOwl:hasOBONamespace>GAZ</oboInOwl:hasOBONamespace>
        <oboInOwl:id>GAZ:00060298</oboInOwl:id>
        <rdfs:label>Lac d&apos;Allos</rdfs:label>
    </owl:NamedIndividual>
    


    <!-- http://purl.obolibrary.org/obo/GAZ_00060299 -->

    <owl:NamedIndividual rdf:about="http://purl.obolibrary.org/obo/GAZ_00060299">
        <obo:RO_0001025 rdf:resource="http://purl.obolibrary.org/obo/GAZ_00060291"/>
        <obo:IAO_0000115>Lacs situee a 2500 m d&apos;altitude dans le massif de Chambeyron en Haute-Ubaye dans les Alpes-de-Haute-Provence.</obo:IAO_0000115>
        <oboInOwl:hasOBONamespace>GAZ</oboInOwl:hasOBONamespace>
        <oboInOwl:id>GAZ:00060299</oboInOwl:id>
        <rdfs:label>Lacs de Marinet</rdfs:label>
    </owl:NamedIndividual>
    


    <!-- http://purl.obolibrary.org/obo/GAZ_00060300 -->

    <owl:NamedIndividual rdf:about="http://purl.obolibrary.org/obo/GAZ_00060300">
        <obo:RO_0001025 rdf:resource="http://purl.obolibrary.org/obo/GAZ_00060291"/>
        <obo:IAO_0000115>Three lacs in the Col de Longet.</obo:IAO_0000115>
        <oboInOwl:hasOBONamespace>GAZ</oboInOwl:hasOBONamespace>
        <oboInOwl:id>GAZ:00060300</oboInOwl:id>
        <rdfs:label>Lacs du Col du Longet</rdfs:label>
    </owl:NamedIndividual>
    


    <!-- http://purl.obolibrary.org/obo/GAZ_00060301 -->

    <owl:NamedIndividual rdf:about="http://purl.obolibrary.org/obo/GAZ_00060301">
        <obo:RO_0001025 rdf:resource="http://purl.obolibrary.org/obo/GAZ_00060291"/>
        <obo:IAO_0000115>A lake in the Ubaye Valley.</obo:IAO_0000115>
        <oboInOwl:hasOBONamespace>GAZ</oboInOwl:hasOBONamespace>
        <oboInOwl:id>GAZ:00060301</oboInOwl:id>
        <rdfs:label>Lac du Lauzet-Ubaye</rdfs:label>
    </owl:NamedIndividual>
    


    <!-- http://purl.obolibrary.org/obo/GAZ_00060302 -->

    <owl:NamedIndividual rdf:about="http://purl.obolibrary.org/obo/GAZ_00060302">
        <obo:RO_0001025 rdf:resource="http://purl.obolibrary.org/obo/GAZ_00060291"/>
        <obo:IAO_0000115>Un lac de montagne qui se situe a une altitude de 2300 m au sein du massif de l&apos;Ubaye, pras de la vallee du meme nom, dans le departement des Alpes-de-Haute-Provence. L&apos;Ubayette y prend sa source.</obo:IAO_0000115>
        <oboInOwl:hasOBONamespace>GAZ</oboInOwl:hasOBONamespace>
        <oboInOwl:id>GAZ:00060302</oboInOwl:id>
        <rdfs:label>Lac du Lauzanier</rdfs:label>
    </owl:NamedIndividual>
    


    <!-- http://purl.obolibrary.org/obo/GAZ_00060305 -->

    <owl:NamedIndividual rdf:about="http://purl.obolibrary.org/obo/GAZ_00060305">
        <obo:RO_0001025 rdf:resource="http://purl.obolibrary.org/obo/GAZ_00060299"/>
        <obo:IAO_0000115>The larger of the two lower Lacs de Marinet.</obo:IAO_0000115>
        <oboInOwl:hasOBONamespace>GAZ</oboInOwl:hasOBONamespace>
        <oboInOwl:id>GAZ:00060305</oboInOwl:id>
        <rdfs:label>Lac-grand du Marinet</rdfs:label>
    </owl:NamedIndividual>
    


    <!-- http://purl.obolibrary.org/obo/GAZ_00060306 -->

    <owl:NamedIndividual rdf:about="http://purl.obolibrary.org/obo/GAZ_00060306">
        <obo:RO_0001025 rdf:resource="http://purl.obolibrary.org/obo/GAZ_00060299"/>
        <obo:IAO_0000115>Two upper Lacs de Marinet.</obo:IAO_0000115>
        <oboInOwl:hasOBONamespace>GAZ</oboInOwl:hasOBONamespace>
        <oboInOwl:id>GAZ:00060306</oboInOwl:id>
        <rdfs:label>Lacs superieurs de Marinet</rdfs:label>
    </owl:NamedIndividual>
    


    <!-- http://purl.obolibrary.org/obo/GAZ_00060307 -->

    <owl:NamedIndividual rdf:about="http://purl.obolibrary.org/obo/GAZ_00060307">
        <obo:RO_0001025 rdf:resource="http://purl.obolibrary.org/obo/GAZ_00060291"/>
        <obo:IAO_0000115>Un lac situe dans la vallee de l&apos;Ubaye, dans les Alpes-de-Haute-Provence, a 2841 m.</obo:IAO_0000115>
        <oboInOwl:hasOBONamespace>GAZ</oboInOwl:hasOBONamespace>
        <oboInOwl:id>GAZ:00060307</oboInOwl:id>
        <rdfs:label>Lac des Neufs Couleurs</rdfs:label>
    </owl:NamedIndividual>
    


    <!-- http://purl.obolibrary.org/obo/GAZ_00060308 -->

    <owl:NamedIndividual rdf:about="http://purl.obolibrary.org/obo/GAZ_00060308">
        <obo:RO_0001025 rdf:resource="http://purl.obolibrary.org/obo/GAZ_00060291"/>
        <obo:IAO_0000115>A lake in the Ubaye Valley.</obo:IAO_0000115>
        <oboInOwl:hasOBONamespace>GAZ</oboInOwl:hasOBONamespace>
        <oboInOwl:id>GAZ:00060308</oboInOwl:id>
        <rdfs:label>Lac de Longet</rdfs:label>
    </owl:NamedIndividual>
    


    <!-- http://purl.obolibrary.org/obo/GAZ_00060309 -->

    <owl:NamedIndividual rdf:about="http://purl.obolibrary.org/obo/GAZ_00060309">
        <obo:RO_0001025 rdf:resource="http://purl.obolibrary.org/obo/GAZ_00060291"/>
        <obo:IAO_0000115>A lake in the Ubaye Valley.</obo:IAO_0000115>
        <oboInOwl:hasOBONamespace>GAZ</oboInOwl:hasOBONamespace>
        <oboInOwl:id>GAZ:00060309</oboInOwl:id>
        <rdfs:label>Lac des Sagnes</rdfs:label>
    </owl:NamedIndividual>
    


    <!-- http://purl.obolibrary.org/obo/GAZ_00060310 -->

    <owl:NamedIndividual rdf:about="http://purl.obolibrary.org/obo/GAZ_00060310">
        <obo:RO_0001025 rdf:resource="http://purl.obolibrary.org/obo/GAZ_00060291"/>
        <obo:IAO_0000115>A lake in the Ubaye Valley.</obo:IAO_0000115>
        <oboInOwl:hasOBONamespace>GAZ</oboInOwl:hasOBONamespace>
        <oboInOwl:id>GAZ:00060310</oboInOwl:id>
        <rdfs:label>Lac Bleu-italien</rdfs:label>
    </owl:NamedIndividual>
    


    <!-- http://purl.obolibrary.org/obo/GAZ_00060311 -->

    <owl:NamedIndividual rdf:about="http://purl.obolibrary.org/obo/GAZ_00060311">
        <obo:RO_0001025 rdf:resource="http://purl.obolibrary.org/obo/GAZ_00060291"/>
        <obo:IAO_0000115>A lake in the Ubaye Valley.</obo:IAO_0000115>
        <oboInOwl:hasOBONamespace>GAZ</oboInOwl:hasOBONamespace>
        <oboInOwl:id>GAZ:00060311</oboInOwl:id>
        <rdfs:label>Lac de l&apos;Etoile</rdfs:label>
    </owl:NamedIndividual>
    


    <!-- http://purl.obolibrary.org/obo/GAZ_00060312 -->

    <owl:NamedIndividual rdf:about="http://purl.obolibrary.org/obo/GAZ_00060312">
        <obo:RO_0001025 rdf:resource="http://purl.obolibrary.org/obo/GAZ_00060291"/>
        <obo:IAO_0000115>A lake in the Ubaye Valley.</obo:IAO_0000115>
        <oboInOwl:hasOBONamespace>GAZ</oboInOwl:hasOBONamespace>
        <oboInOwl:id>GAZ:00060312</oboInOwl:id>
        <rdfs:label>Lac Noir-de-Chambeyron</rdfs:label>
    </owl:NamedIndividual>
    


    <!-- http://purl.obolibrary.org/obo/GAZ_00060313 -->

    <owl:NamedIndividual rdf:about="http://purl.obolibrary.org/obo/GAZ_00060313">
        <obo:RO_0001025 rdf:resource="http://purl.obolibrary.org/obo/GAZ_00060291"/>
        <obo:IAO_0000115>A lake in the Ubaye Valley.</obo:IAO_0000115>
        <oboInOwl:hasOBONamespace>GAZ</oboInOwl:hasOBONamespace>
        <oboInOwl:id>GAZ:00060313</oboInOwl:id>
        <rdfs:label>Lac de Terre-Pleine</rdfs:label>
    </owl:NamedIndividual>
    


    <!-- http://purl.obolibrary.org/obo/GAZ_00060314 -->

    <owl:NamedIndividual rdf:about="http://purl.obolibrary.org/obo/GAZ_00060314">
        <obo:RO_0001025 rdf:resource="http://purl.obolibrary.org/obo/GAZ_00060291"/>
        <obo:IAO_0000115>A lake in the Ubaye Valley.</obo:IAO_0000115>
        <oboInOwl:hasOBONamespace>GAZ</oboInOwl:hasOBONamespace>
        <oboInOwl:id>GAZ:00060314</oboInOwl:id>
        <rdfs:label>Lac Vert-de-Morticet</rdfs:label>
    </owl:NamedIndividual>
    


    <!-- http://purl.obolibrary.org/obo/GAZ_00060315 -->

    <owl:NamedIndividual rdf:about="http://purl.obolibrary.org/obo/GAZ_00060315">
        <obo:RO_0001025 rdf:resource="http://purl.obolibrary.org/obo/GAZ_00060291"/>
        <obo:IAO_0000115>A lake in the Ubaye Valley.</obo:IAO_0000115>
        <oboInOwl:hasOBONamespace>GAZ</oboInOwl:hasOBONamespace>
        <oboInOwl:id>GAZ:00060315</oboInOwl:id>
        <rdfs:label>Lac Bleu</rdfs:label>
    </owl:NamedIndividual>
    


    <!-- http://purl.obolibrary.org/obo/GAZ_00060316 -->

    <owl:NamedIndividual rdf:about="http://purl.obolibrary.org/obo/GAZ_00060316">
        <obo:RO_0001025 rdf:resource="http://purl.obolibrary.org/obo/GAZ_00060291"/>
        <obo:IAO_0000115>A lake in the Ubaye Valley.</obo:IAO_0000115>
        <oboInOwl:hasOBONamespace>GAZ</oboInOwl:hasOBONamespace>
        <oboInOwl:id>GAZ:00060316</oboInOwl:id>
        <rdfs:label>Lac Rond-de-Chambeyron</rdfs:label>
    </owl:NamedIndividual>
    


    <!-- http://purl.obolibrary.org/obo/GAZ_00060317 -->

    <owl:NamedIndividual rdf:about="http://purl.obolibrary.org/obo/GAZ_00060317">
        <obo:RO_0001025 rdf:resource="http://purl.obolibrary.org/obo/GAZ_00060291"/>
        <obo:IAO_0000115>A lake in the Ubaye Valley.</obo:IAO_0000115>
        <oboInOwl:hasOBONamespace>GAZ</oboInOwl:hasOBONamespace>
        <oboInOwl:id>GAZ:00060317</oboInOwl:id>
        <rdfs:label>Lac de la Noire</rdfs:label>
    </owl:NamedIndividual>
    


    <!-- http://purl.obolibrary.org/obo/GAZ_00060318 -->

    <owl:NamedIndividual rdf:about="http://purl.obolibrary.org/obo/GAZ_00060318">
        <obo:RO_0001025 rdf:resource="http://purl.obolibrary.org/obo/GAZ_00009679"/>
        <obo:IAO_0000115>A national park consisting of a central uninhabited zone comprising seven valleys - Roya, Bevera, Vesubie, Tinee, Haut Var/Cians (in the Alpes-Maritimes) plus Verdon and Ubaye (in the Alpes-de-Haute-Provence) - and a peripheral zone comprising 28 villages.</obo:IAO_0000115>
        <oboInOwl:hasOBONamespace>GAZ</oboInOwl:hasOBONamespace>
        <oboInOwl:id>GAZ:00060318</oboInOwl:id>
        <rdfs:label>Parc national du Mercantour</rdfs:label>
    </owl:NamedIndividual>
    


    <!-- http://purl.obolibrary.org/obo/GAZ_00060330 -->

    <owl:NamedIndividual rdf:about="http://purl.obolibrary.org/obo/GAZ_00060330">
        <obo:RO_0001025 rdf:resource="http://purl.obolibrary.org/obo/GAZ_00060608"/>
        <obo:IAO_0000115>A glacial lake.</obo:IAO_0000115>
        <oboInOwl:hasOBONamespace>GAZ</oboInOwl:hasOBONamespace>
        <oboInOwl:id>GAZ:00060330</oboInOwl:id>
        <rdfs:label>Lac Autier</rdfs:label>
    </owl:NamedIndividual>
    


    <!-- http://purl.obolibrary.org/obo/GAZ_00060391 -->

    <owl:NamedIndividual rdf:about="http://purl.obolibrary.org/obo/GAZ_00060391">
        <obo:RO_0001025 rdf:resource="http://purl.obolibrary.org/obo/GAZ_00009675"/>
        <obo:IAO_0000115>A mountain range in the Dauphine Alps in southeast France. The southern end of the range forms the eastern wall of the mountains that surround the city of Grenoble. It is principaly in the Department of Isere, but the NW is in the Department of Savoie.</obo:IAO_0000115>
        <oboInOwl:hasOBONamespace>GAZ</oboInOwl:hasOBONamespace>
        <oboInOwl:id>GAZ:00060391</oboInOwl:id>
        <rdfs:label>La chaine de Belledonne</rdfs:label>
    </owl:NamedIndividual>
    


    <!-- http://purl.obolibrary.org/obo/GAZ_00060394 -->

    <owl:NamedIndividual rdf:about="http://purl.obolibrary.org/obo/GAZ_00060394">
        <obo:RO_0001025 rdf:resource="http://purl.obolibrary.org/obo/GAZ_00060391"/>
        <obo:IAO_0000115>A lake in La chaine de Belledonne at 2124m.</obo:IAO_0000115>
        <oboInOwl:hasOBONamespace>GAZ</oboInOwl:hasOBONamespace>
        <oboInOwl:id>GAZ:00060394</oboInOwl:id>
        <rdfs:label>Lac Blanc</rdfs:label>
    </owl:NamedIndividual>
    


    <!-- http://purl.obolibrary.org/obo/GAZ_00060395 -->

    <owl:NamedIndividual rdf:about="http://purl.obolibrary.org/obo/GAZ_00060395">
        <obo:RO_0001025 rdf:resource="http://purl.obolibrary.org/obo/GAZ_00060391"/>
        <obo:IAO_0000115>A lake in La chaine de Belledonne.</obo:IAO_0000115>
        <oboInOwl:hasOBONamespace>GAZ</oboInOwl:hasOBONamespace>
        <oboInOwl:id>GAZ:00060395</oboInOwl:id>
        <rdfs:label>Lac de la Croix</rdfs:label>
    </owl:NamedIndividual>
    


    <!-- http://purl.obolibrary.org/obo/GAZ_00060396 -->

    <owl:NamedIndividual rdf:about="http://purl.obolibrary.org/obo/GAZ_00060396">
        <obo:RO_0001025 rdf:resource="http://purl.obolibrary.org/obo/GAZ_00060391"/>
        <obo:IAO_0000115>A lake in La chaine de Belledonne.</obo:IAO_0000115>
        <oboInOwl:hasOBONamespace>GAZ</oboInOwl:hasOBONamespace>
        <oboInOwl:id>GAZ:00060396</oboInOwl:id>
        <rdfs:label>Lac Merlat</rdfs:label>
    </owl:NamedIndividual>
    


    <!-- http://purl.obolibrary.org/obo/GAZ_00060398 -->

    <owl:NamedIndividual rdf:about="http://purl.obolibrary.org/obo/GAZ_00060398">
        <obo:RO_0001025 rdf:resource="http://purl.obolibrary.org/obo/GAZ_00060391"/>
        <obo:IAO_0000115>Un lac de France situe dans les Alpes, dans le sud de la chaine de Belledonne, a proximite de la station de sports d&apos;hiver de Chamrousse.</obo:IAO_0000115>
        <oboInOwl:hasOBONamespace>GAZ</oboInOwl:hasOBONamespace>
        <oboInOwl:id>GAZ:00060398</oboInOwl:id>
        <rdfs:label>Lac Achard</rdfs:label>
    </owl:NamedIndividual>
    


    <!-- http://purl.obolibrary.org/obo/GAZ_00060399 -->

    <owl:NamedIndividual rdf:about="http://purl.obolibrary.org/obo/GAZ_00060399">
        <obo:RO_0001025 rdf:resource="http://purl.obolibrary.org/obo/GAZ_00060391"/>
        <obo:IAO_0000115>A lake in La chaine de Belledonne.</obo:IAO_0000115>
        <oboInOwl:hasOBONamespace>GAZ</oboInOwl:hasOBONamespace>
        <oboInOwl:id>GAZ:00060399</oboInOwl:id>
        <rdfs:label>Lac de la Folle</rdfs:label>
    </owl:NamedIndividual>
    


    <!-- http://purl.obolibrary.org/obo/GAZ_00060400 -->

    <owl:NamedIndividual rdf:about="http://purl.obolibrary.org/obo/GAZ_00060400">
        <obo:RO_0001025 rdf:resource="http://purl.obolibrary.org/obo/GAZ_00060391"/>
        <obo:IAO_0000115>A lake in La chaine de Belledonne.</obo:IAO_0000115>
        <oboInOwl:hasOBONamespace>GAZ</oboInOwl:hasOBONamespace>
        <oboInOwl:id>GAZ:00060400</oboInOwl:id>
        <rdfs:label>Lac de la Sitre</rdfs:label>
    </owl:NamedIndividual>
    


    <!-- http://purl.obolibrary.org/obo/GAZ_00060401 -->

    <owl:NamedIndividual rdf:about="http://purl.obolibrary.org/obo/GAZ_00060401">
        <obo:RO_0001025 rdf:resource="http://purl.obolibrary.org/obo/GAZ_00060391"/>
        <obo:IAO_0000115>A lake in La chaine de Belledonne at 2268m.</obo:IAO_0000115>
        <oboInOwl:hasOBONamespace>GAZ</oboInOwl:hasOBONamespace>
        <oboInOwl:id>GAZ:00060401</oboInOwl:id>
        <rdfs:label>Lac Noir</rdfs:label>
    </owl:NamedIndividual>
    


    <!-- http://purl.obolibrary.org/obo/GAZ_00060404 -->

    <owl:NamedIndividual rdf:about="http://purl.obolibrary.org/obo/GAZ_00060404">
        <obo:RO_0001025 rdf:resource="http://purl.obolibrary.org/obo/GAZ_00060391"/>
    </owl:NamedIndividual>
    


    <!-- http://purl.obolibrary.org/obo/GAZ_00060407 -->

    <owl:NamedIndividual rdf:about="http://purl.obolibrary.org/obo/GAZ_00060407">
        <obo:RO_0001025 rdf:resource="http://purl.obolibrary.org/obo/GAZ_00060391"/>
        <obo:IAO_0000115>A lake in La chaine de Belledonne.</obo:IAO_0000115>
        <oboInOwl:hasOBONamespace>GAZ</oboInOwl:hasOBONamespace>
        <oboInOwl:id>GAZ:00060407</oboInOwl:id>
        <rdfs:label>Lac des Balmettes</rdfs:label>
    </owl:NamedIndividual>
    


    <!-- http://purl.obolibrary.org/obo/GAZ_00060408 -->

    <owl:NamedIndividual rdf:about="http://purl.obolibrary.org/obo/GAZ_00060408">
        <obo:RO_0001025 rdf:resource="http://purl.obolibrary.org/obo/GAZ_00060391"/>
        <obo:IAO_0000115>A lake in La chaine de Belledonne.</obo:IAO_0000115>
        <oboInOwl:hasOBONamespace>GAZ</oboInOwl:hasOBONamespace>
        <oboInOwl:id>GAZ:00060408</oboInOwl:id>
        <rdfs:label>Lac Longet</rdfs:label>
    </owl:NamedIndividual>
    


    <!-- http://purl.obolibrary.org/obo/GAZ_00060410 -->

    <owl:NamedIndividual rdf:about="http://purl.obolibrary.org/obo/GAZ_00060410">
        <obo:RO_0001025 rdf:resource="http://purl.obolibrary.org/obo/GAZ_00060391"/>
    </owl:NamedIndividual>
    


    <!-- http://purl.obolibrary.org/obo/GAZ_00060411 -->

    <owl:NamedIndividual rdf:about="http://purl.obolibrary.org/obo/GAZ_00060411">
        <obo:RO_0001025 rdf:resource="http://purl.obolibrary.org/obo/GAZ_00060391"/>
        <obo:IAO_0000115>A lake in La chaine de Belledonne.</obo:IAO_0000115>
        <oboInOwl:hasOBONamespace>GAZ</oboInOwl:hasOBONamespace>
        <oboInOwl:id>GAZ:00060411</oboInOwl:id>
        <rdfs:label>Lac de Belledonne</rdfs:label>
    </owl:NamedIndividual>
    


    <!-- http://purl.obolibrary.org/obo/GAZ_00060413 -->

    <owl:NamedIndividual rdf:about="http://purl.obolibrary.org/obo/GAZ_00060413">
        <obo:RO_0001025 rdf:resource="http://purl.obolibrary.org/obo/GAZ_00060391"/>
        <obo:IAO_0000115>A lake in La chaine de Belledonne at 2161m.</obo:IAO_0000115>
        <oboInOwl:hasOBONamespace>GAZ</oboInOwl:hasOBONamespace>
        <oboInOwl:id>GAZ:00060413</oboInOwl:id>
        <rdfs:label>Lac Blanc</rdfs:label>
    </owl:NamedIndividual>
    


    <!-- http://purl.obolibrary.org/obo/GAZ_00060414 -->

    <owl:NamedIndividual rdf:about="http://purl.obolibrary.org/obo/GAZ_00060414">
        <obo:RO_0001025 rdf:resource="http://purl.obolibrary.org/obo/GAZ_00060391"/>
        <obo:IAO_0000115>A lake in La chaine de Belledonne.</obo:IAO_0000115>
        <oboInOwl:hasOBONamespace>GAZ</oboInOwl:hasOBONamespace>
        <oboInOwl:id>GAZ:00060414</oboInOwl:id>
        <rdfs:label>Lac de Crop</rdfs:label>
    </owl:NamedIndividual>
    


    <!-- http://purl.obolibrary.org/obo/GAZ_00060416 -->

    <owl:NamedIndividual rdf:about="http://purl.obolibrary.org/obo/GAZ_00060416">
        <obo:RO_0001025 rdf:resource="http://purl.obolibrary.org/obo/GAZ_00060391"/>
        <obo:IAO_0000115>A lake in La chaine de Belledonne.</obo:IAO_0000115>
        <oboInOwl:hasOBONamespace>GAZ</oboInOwl:hasOBONamespace>
        <oboInOwl:id>GAZ:00060416</oboInOwl:id>
        <rdfs:label>Lac du Crozet</rdfs:label>
    </owl:NamedIndividual>
    


    <!-- http://purl.obolibrary.org/obo/GAZ_00060417 -->

    <owl:NamedIndividual rdf:about="http://purl.obolibrary.org/obo/GAZ_00060417">
        <obo:RO_0001025 rdf:resource="http://purl.obolibrary.org/obo/GAZ_00060391"/>
        <obo:IAO_0000115>A lake in La chaine de Belledonne.</obo:IAO_0000115>
        <oboInOwl:hasOBONamespace>GAZ</oboInOwl:hasOBONamespace>
        <oboInOwl:id>GAZ:00060417</oboInOwl:id>
        <rdfs:label>Lac du Grand Domenon</rdfs:label>
    </owl:NamedIndividual>
    


    <!-- http://purl.obolibrary.org/obo/GAZ_00060418 -->

    <owl:NamedIndividual rdf:about="http://purl.obolibrary.org/obo/GAZ_00060418">
        <obo:RO_0001025 rdf:resource="http://purl.obolibrary.org/obo/GAZ_00060391"/>
        <obo:IAO_0000115>A lake in La chaine de Belledonne.</obo:IAO_0000115>
        <oboInOwl:hasOBONamespace>GAZ</oboInOwl:hasOBONamespace>
        <oboInOwl:id>GAZ:00060418</oboInOwl:id>
        <rdfs:label>Lac Claret</rdfs:label>
    </owl:NamedIndividual>
    


    <!-- http://purl.obolibrary.org/obo/GAZ_00060419 -->

    <owl:NamedIndividual rdf:about="http://purl.obolibrary.org/obo/GAZ_00060419">
        <obo:RO_0001025 rdf:resource="http://purl.obolibrary.org/obo/GAZ_00060391"/>
        <obo:IAO_0000115>A lake in La chaine de Belledonne.</obo:IAO_0000115>
        <oboInOwl:hasOBONamespace>GAZ</oboInOwl:hasOBONamespace>
        <oboInOwl:id>GAZ:00060419</oboInOwl:id>
        <rdfs:label>Lac du Petit Domenon</rdfs:label>
    </owl:NamedIndividual>
    


    <!-- http://purl.obolibrary.org/obo/GAZ_00060420 -->

    <owl:NamedIndividual rdf:about="http://purl.obolibrary.org/obo/GAZ_00060420">
        <obo:RO_0001025 rdf:resource="http://purl.obolibrary.org/obo/GAZ_00060391"/>
        <obo:IAO_0000115>A lake in La chaine de Belledonne at 2161m.</obo:IAO_0000115>
        <oboInOwl:hasOBONamespace>GAZ</oboInOwl:hasOBONamespace>
        <oboInOwl:id>GAZ:00060420</oboInOwl:id>
        <rdfs:label>Lac de la Coche</rdfs:label>
    </owl:NamedIndividual>
    


    <!-- http://purl.obolibrary.org/obo/GAZ_00060421 -->

    <owl:NamedIndividual rdf:about="http://purl.obolibrary.org/obo/GAZ_00060421">
        <obo:RO_0001025 rdf:resource="http://purl.obolibrary.org/obo/GAZ_00059214"/>
        <obo:IAO_0000115>A lake in Isere. Situes au Nord-Est de l&apos;Alpe d&apos;Huez dans le massif des Grandes Rousses.</obo:IAO_0000115>
        <oboInOwl:hasOBONamespace>GAZ</oboInOwl:hasOBONamespace>
        <oboInOwl:id>GAZ:00060421</oboInOwl:id>
        <rdfs:label>Lac Besson</rdfs:label>
    </owl:NamedIndividual>
    


    <!-- http://purl.obolibrary.org/obo/GAZ_00060422 -->

    <owl:NamedIndividual rdf:about="http://purl.obolibrary.org/obo/GAZ_00060422">
        <obo:RO_0001025 rdf:resource="http://purl.obolibrary.org/obo/GAZ_00060391"/>
        <obo:IAO_0000115>A lake in La chaine de Belledonne.</obo:IAO_0000115>
        <oboInOwl:hasOBONamespace>GAZ</oboInOwl:hasOBONamespace>
        <oboInOwl:id>GAZ:00060422</oboInOwl:id>
        <rdfs:label>Lac de Croz</rdfs:label>
    </owl:NamedIndividual>
    


    <!-- http://purl.obolibrary.org/obo/GAZ_00060423 -->

    <owl:NamedIndividual rdf:about="http://purl.obolibrary.org/obo/GAZ_00060423">
        <obo:RO_0001025 rdf:resource="http://purl.obolibrary.org/obo/GAZ_00060391"/>
        <obo:IAO_0000115>A lake in La chaine de Belledonne.</obo:IAO_0000115>
        <oboInOwl:hasOBONamespace>GAZ</oboInOwl:hasOBONamespace>
        <oboInOwl:id>GAZ:00060423</oboInOwl:id>
        <rdfs:label>Lac du Flumet</rdfs:label>
    </owl:NamedIndividual>
    


    <!-- http://purl.obolibrary.org/obo/GAZ_00060424 -->

    <owl:NamedIndividual rdf:about="http://purl.obolibrary.org/obo/GAZ_00060424">
        <obo:RO_0001025 rdf:resource="http://purl.obolibrary.org/obo/GAZ_00059214"/>
        <obo:IAO_0000115>A lake in the Grandes Rousses in Iseres.</obo:IAO_0000115>
        <oboInOwl:hasOBONamespace>GAZ</oboInOwl:hasOBONamespace>
        <oboInOwl:id>GAZ:00060424</oboInOwl:id>
        <rdfs:label>Lac de la Fare</rdfs:label>
    </owl:NamedIndividual>
    


    <!-- http://purl.obolibrary.org/obo/GAZ_00060425 -->

    <owl:NamedIndividual rdf:about="http://purl.obolibrary.org/obo/GAZ_00060425">
        <obo:RO_0001025 rdf:resource="http://purl.obolibrary.org/obo/GAZ_00059214"/>
        <obo:IAO_0000115>A lake in the Grandes Rousses in Iseres.</obo:IAO_0000115>
        <oboInOwl:hasOBONamespace>GAZ</oboInOwl:hasOBONamespace>
        <oboInOwl:id>GAZ:00060425</oboInOwl:id>
        <rdfs:label>Lac Faucille</rdfs:label>
    </owl:NamedIndividual>
    


    <!-- http://purl.obolibrary.org/obo/GAZ_00060426 -->

    <owl:NamedIndividual rdf:about="http://purl.obolibrary.org/obo/GAZ_00060426">
        <obo:RO_0001025 rdf:resource="http://purl.obolibrary.org/obo/GAZ_00060391"/>
        <obo:IAO_0000115>A lake in La chaine de Belledonne.</obo:IAO_0000115>
        <oboInOwl:hasOBONamespace>GAZ</oboInOwl:hasOBONamespace>
        <oboInOwl:id>GAZ:00060426</oboInOwl:id>
        <rdfs:label>Lac de la Grande-Sitre</rdfs:label>
    </owl:NamedIndividual>
    


    <!-- http://purl.obolibrary.org/obo/GAZ_00060427 -->

    <owl:NamedIndividual rdf:about="http://purl.obolibrary.org/obo/GAZ_00060427">
        <obo:RO_0001025 rdf:resource="http://purl.obolibrary.org/obo/GAZ_00059214"/>
        <obo:IAO_0000115>A lake in the Grandes Rousses in Iseres.</obo:IAO_0000115>
        <oboInOwl:hasOBONamespace>GAZ</oboInOwl:hasOBONamespace>
        <oboInOwl:id>GAZ:00060427</oboInOwl:id>
        <rdfs:label>Lac Guichard</rdfs:label>
    </owl:NamedIndividual>
    


    <!-- http://purl.obolibrary.org/obo/GAZ_00060429 -->

    <owl:NamedIndividual rdf:about="http://purl.obolibrary.org/obo/GAZ_00060429">
        <obo:RO_0001025 rdf:resource="http://purl.obolibrary.org/obo/GAZ_00059214"/>
        <obo:IAO_0000115>A lake in the Grandes Rousses in Iseres.</obo:IAO_0000115>
        <oboInOwl:hasOBONamespace>GAZ</oboInOwl:hasOBONamespace>
        <oboInOwl:id>GAZ:00060429</oboInOwl:id>
        <rdfs:label>Lac du Milieu</rdfs:label>
    </owl:NamedIndividual>
    


    <!-- http://purl.obolibrary.org/obo/GAZ_00060430 -->

    <owl:NamedIndividual rdf:about="http://purl.obolibrary.org/obo/GAZ_00060430">
        <obo:RO_0001025 rdf:resource="http://purl.obolibrary.org/obo/GAZ_00059214"/>
        <obo:IAO_0000115>A lake in the Grandes Rousses in Iseres.</obo:IAO_0000115>
        <oboInOwl:hasOBONamespace>GAZ</oboInOwl:hasOBONamespace>
        <oboInOwl:id>GAZ:00060430</oboInOwl:id>
        <rdfs:label>Lac Noir</rdfs:label>
    </owl:NamedIndividual>
    


    <!-- http://purl.obolibrary.org/obo/GAZ_00060431 -->

    <owl:NamedIndividual rdf:about="http://purl.obolibrary.org/obo/GAZ_00060431">
        <obo:RO_0001025 rdf:resource="http://purl.obolibrary.org/obo/GAZ_00059214"/>
        <obo:IAO_0000115>A lake in the Grandes Rousses in Iseres. Impounded by Barrage du Verney.</obo:IAO_0000115>
        <oboInOwl:hasOBONamespace>GAZ</oboInOwl:hasOBONamespace>
        <oboInOwl:id>GAZ:00060431</oboInOwl:id>
        <rdfs:label>Lac du Verney</rdfs:label>
    </owl:NamedIndividual>
    


    <!-- http://purl.obolibrary.org/obo/GAZ_00060432 -->

    <owl:NamedIndividual rdf:about="http://purl.obolibrary.org/obo/GAZ_00060432">
        <obo:RO_0001025 rdf:resource="http://purl.obolibrary.org/obo/GAZ_00059214"/>
        <obo:IAO_0000115>A lake in the Grandes Rousses in Iseres.</obo:IAO_0000115>
        <oboInOwl:hasOBONamespace>GAZ</oboInOwl:hasOBONamespace>
        <oboInOwl:id>GAZ:00060432</oboInOwl:id>
        <rdfs:label>Lac Potet</rdfs:label>
    </owl:NamedIndividual>
    


    <!-- http://purl.obolibrary.org/obo/GAZ_00060433 -->

    <owl:NamedIndividual rdf:about="http://purl.obolibrary.org/obo/GAZ_00060433">
        <obo:RO_0001025 rdf:resource="http://purl.obolibrary.org/obo/GAZ_00059237"/>
        <obo:IAO_0000115>A lake in the Massif du Taillefer.</obo:IAO_0000115>
        <oboInOwl:hasOBONamespace>GAZ</oboInOwl:hasOBONamespace>
        <oboInOwl:id>GAZ:00060433</oboInOwl:id>
        <rdfs:label>Lac Brouffier</rdfs:label>
    </owl:NamedIndividual>
    


    <!-- http://purl.obolibrary.org/obo/GAZ_00060434 -->

    <owl:NamedIndividual rdf:about="http://purl.obolibrary.org/obo/GAZ_00060434">
        <obo:RO_0001025 rdf:resource="http://purl.obolibrary.org/obo/GAZ_00059237"/>
        <obo:IAO_0000115>Un lac de France situe dans les Alpes, en Isere, dans le massif du Taillefer.</obo:IAO_0000115>
        <oboInOwl:hasOBONamespace>GAZ</oboInOwl:hasOBONamespace>
        <oboInOwl:id>GAZ:00060434</oboInOwl:id>
        <rdfs:label>Lac Fourchu</rdfs:label>
    </owl:NamedIndividual>
    


    <!-- http://purl.obolibrary.org/obo/GAZ_00060440 -->

    <owl:NamedIndividual rdf:about="http://purl.obolibrary.org/obo/GAZ_00060440">
        <obo:RO_0001025 rdf:resource="http://purl.obolibrary.org/obo/GAZ_00060256"/>
        <obo:IAO_0000115>Un lac situe a 1530 m, dans la vallee du Veneon. C&apos;est le plus grand lac du Massif des Ecrins (Isere), en fait un versant de l&apos;Oisans.</obo:IAO_0000115>
        <oboInOwl:hasOBONamespace>GAZ</oboInOwl:hasOBONamespace>
        <oboInOwl:id>GAZ:00060440</oboInOwl:id>
        <rdfs:label>Lac du Lauvitel</rdfs:label>
    </owl:NamedIndividual>
    


    <!-- http://purl.obolibrary.org/obo/GAZ_00060441 -->

    <owl:NamedIndividual rdf:about="http://purl.obolibrary.org/obo/GAZ_00060441">
        <obo:RO_0001025 rdf:resource="http://purl.obolibrary.org/obo/GAZ_00060256"/>
        <obo:IAO_0000115>Un petit lac de montagne dans le departement des Hautes-Alpes, a l&apos;ouest de La Grave. Le lac est situe sur le Plateau d&apos;En Paris (ou Enparis) a 2450 m.</obo:IAO_0000115>
        <oboInOwl:hasOBONamespace>GAZ</oboInOwl:hasOBONamespace>
        <oboInOwl:id>GAZ:00060441</oboInOwl:id>
        <rdfs:label>Lac Lerie</rdfs:label>
    </owl:NamedIndividual>
    


    <!-- http://purl.obolibrary.org/obo/GAZ_00060444 -->

    <owl:NamedIndividual rdf:about="http://purl.obolibrary.org/obo/GAZ_00060444">
        <obo:RO_0001025 rdf:resource="http://purl.obolibrary.org/obo/GAZ_00060256"/>
        <obo:IAO_0000115>A glacial lake in the Massif des Ecrins, in Isere.</obo:IAO_0000115>
        <oboInOwl:hasOBONamespace>GAZ</oboInOwl:hasOBONamespace>
        <oboInOwl:id>GAZ:00060444</oboInOwl:id>
        <rdfs:label>Lac de la Muzelle</rdfs:label>
    </owl:NamedIndividual>
    


    <!-- http://purl.obolibrary.org/obo/GAZ_00060445 -->

    <owl:NamedIndividual rdf:about="http://purl.obolibrary.org/obo/GAZ_00060445">
        <obo:RO_0001025 rdf:resource="http://purl.obolibrary.org/obo/GAZ_00060256"/>
        <obo:IAO_0000115>A lake in the Massif des Ecrins, in Isere.</obo:IAO_0000115>
        <oboInOwl:hasOBONamespace>GAZ</oboInOwl:hasOBONamespace>
        <oboInOwl:id>GAZ:00060445</oboInOwl:id>
        <rdfs:label>Lac Noir d&apos;Emparis</rdfs:label>
    </owl:NamedIndividual>
    


    <!-- http://purl.obolibrary.org/obo/GAZ_00060446 -->

    <owl:NamedIndividual rdf:about="http://purl.obolibrary.org/obo/GAZ_00060446">
        <obo:RO_0001025 rdf:resource="http://purl.obolibrary.org/obo/GAZ_00060256"/>
        <obo:IAO_0000115>A lake in the Massif des Ecrins, in Isere.</obo:IAO_0000115>
        <oboInOwl:hasOBONamespace>GAZ</oboInOwl:hasOBONamespace>
        <oboInOwl:id>GAZ:00060446</oboInOwl:id>
        <rdfs:label>Lac du Plan</rdfs:label>
    </owl:NamedIndividual>
    


    <!-- http://purl.obolibrary.org/obo/GAZ_00060447 -->

    <owl:NamedIndividual rdf:about="http://purl.obolibrary.org/obo/GAZ_00060447">
        <obo:RO_0001025 rdf:resource="http://purl.obolibrary.org/obo/GAZ_00059237"/>
        <obo:IAO_0000115>A lake in the Massif du Taillefer.</obo:IAO_0000115>
        <oboInOwl:hasOBONamespace>GAZ</oboInOwl:hasOBONamespace>
        <oboInOwl:id>GAZ:00060447</oboInOwl:id>
        <rdfs:label>Lac du Poursollet</rdfs:label>
    </owl:NamedIndividual>
    


    <!-- http://purl.obolibrary.org/obo/GAZ_00060448 -->

    <owl:NamedIndividual rdf:about="http://purl.obolibrary.org/obo/GAZ_00060448">
        <obo:RO_0001025 rdf:resource="http://purl.obolibrary.org/obo/GAZ_00060256"/>
        <obo:IAO_0000115>A lake in the Massif des Ecrins, in Isere.</obo:IAO_0000115>
        <oboInOwl:hasOBONamespace>GAZ</oboInOwl:hasOBONamespace>
        <oboInOwl:id>GAZ:00060448</oboInOwl:id>
        <rdfs:label>Lac du Pontet</rdfs:label>
    </owl:NamedIndividual>
    


    <!-- http://purl.obolibrary.org/obo/GAZ_00060500 -->

    <owl:NamedIndividual rdf:about="http://purl.obolibrary.org/obo/GAZ_00060500">
        <obo:RO_0001025 rdf:resource="http://purl.obolibrary.org/obo/GAZ_00008200"/>
        <obo:IAO_0000115>A mountain range in the Graian Alps in the western part of the Alps.</obo:IAO_0000115>
        <oboInOwl:hasOBONamespace>GAZ</oboInOwl:hasOBONamespace>
        <oboInOwl:id>GAZ:00060500</oboInOwl:id>
        <rdfs:label>Masiff de Vanoise</rdfs:label>
    </owl:NamedIndividual>
    


    <!-- http://purl.obolibrary.org/obo/GAZ_00060501 -->

    <owl:NamedIndividual rdf:about="http://purl.obolibrary.org/obo/GAZ_00060501">
        <obo:RO_0001025 rdf:resource="http://purl.obolibrary.org/obo/GAZ_00060500"/>
        <obo:IAO_0000115>A lake in the Masiff de Vanoise.</obo:IAO_0000115>
        <oboInOwl:hasOBONamespace>GAZ</oboInOwl:hasOBONamespace>
        <oboInOwl:id>GAZ:00060501</oboInOwl:id>
        <rdfs:label>Lac de Chasseforet</rdfs:label>
    </owl:NamedIndividual>
    


    <!-- http://purl.obolibrary.org/obo/GAZ_00060502 -->

    <owl:NamedIndividual rdf:about="http://purl.obolibrary.org/obo/GAZ_00060502">
        <obo:RO_0001025 rdf:resource="http://purl.obolibrary.org/obo/GAZ_00060500"/>
        <obo:IAO_0000115>A lake in the Masiff de Vanoise.</obo:IAO_0000115>
        <oboInOwl:hasOBONamespace>GAZ</oboInOwl:hasOBONamespace>
        <oboInOwl:id>GAZ:00060502</oboInOwl:id>
        <rdfs:label>Lac Blanc [Doron]</rdfs:label>
    </owl:NamedIndividual>
    


    <!-- http://purl.obolibrary.org/obo/GAZ_00060503 -->

    <owl:NamedIndividual rdf:about="http://purl.obolibrary.org/obo/GAZ_00060503">
        <obo:RO_0001025 rdf:resource="http://purl.obolibrary.org/obo/GAZ_00060500"/>
        <obo:IAO_0000115>A lake in the Masiff de Vanoise.</obo:IAO_0000115>
        <oboInOwl:hasOBONamespace>GAZ</oboInOwl:hasOBONamespace>
        <oboInOwl:id>GAZ:00060503</oboInOwl:id>
        <rdfs:label>Lac des Assiettes</rdfs:label>
    </owl:NamedIndividual>
    


    <!-- http://purl.obolibrary.org/obo/GAZ_00060504 -->

    <owl:NamedIndividual rdf:about="http://purl.obolibrary.org/obo/GAZ_00060504">
        <obo:RO_0001025 rdf:resource="http://purl.obolibrary.org/obo/GAZ_00060500"/>
        <obo:IAO_0000115>A lake in the Masiff de Vanoise.</obo:IAO_0000115>
        <oboInOwl:hasOBONamespace>GAZ</oboInOwl:hasOBONamespace>
        <oboInOwl:id>GAZ:00060504</oboInOwl:id>
        <rdfs:label>Lac Blanc [Infernet]</rdfs:label>
    </owl:NamedIndividual>
    


    <!-- http://purl.obolibrary.org/obo/GAZ_00060505 -->

    <owl:NamedIndividual rdf:about="http://purl.obolibrary.org/obo/GAZ_00060505">
        <obo:RO_0001025 rdf:resource="http://purl.obolibrary.org/obo/GAZ_00060500"/>
        <obo:IAO_0000115>A lake in the Masiff de Vanoise.</obo:IAO_0000115>
        <oboInOwl:hasOBONamespace>GAZ</oboInOwl:hasOBONamespace>
        <oboInOwl:id>GAZ:00060505</oboInOwl:id>
        <rdfs:label>Lac de l&apos;Arpont</rdfs:label>
    </owl:NamedIndividual>
    


    <!-- http://purl.obolibrary.org/obo/GAZ_00060506 -->

    <owl:NamedIndividual rdf:about="http://purl.obolibrary.org/obo/GAZ_00060506">
        <obo:RO_0001025 rdf:resource="http://purl.obolibrary.org/obo/GAZ_00060500"/>
        <obo:IAO_0000115>A lake in the Masiff de Vanoise.</obo:IAO_0000115>
        <oboInOwl:hasOBONamespace>GAZ</oboInOwl:hasOBONamespace>
        <oboInOwl:id>GAZ:00060506</oboInOwl:id>
        <rdfs:label>Lac de la Gliere</rdfs:label>
    </owl:NamedIndividual>
    


    <!-- http://purl.obolibrary.org/obo/GAZ_00060507 -->

    <owl:NamedIndividual rdf:about="http://purl.obolibrary.org/obo/GAZ_00060507">
        <obo:RO_0001025 rdf:resource="http://purl.obolibrary.org/obo/GAZ_00060500"/>
        <obo:IAO_0000115>A lake in the Masiff de Vanoise.</obo:IAO_0000115>
        <oboInOwl:hasOBONamespace>GAZ</oboInOwl:hasOBONamespace>
        <oboInOwl:id>GAZ:00060507</oboInOwl:id>
        <rdfs:label>Lac le Lou</rdfs:label>
    </owl:NamedIndividual>
    


    <!-- http://purl.obolibrary.org/obo/GAZ_00060508 -->

    <owl:NamedIndividual rdf:about="http://purl.obolibrary.org/obo/GAZ_00060508">
        <obo:RO_0001025 rdf:resource="http://purl.obolibrary.org/obo/GAZ_00060500"/>
        <obo:IAO_0000115>Un parc national situe dans le departement de la Savoie dans le massif du meme nom qui se situe entre la vallee de l&apos;Isere, la Tarentaise au nord et celle de l&apos;Arc, la Maurienne au sud. Il jouxte le Parc National Italien du Grand-Paradis le long de la frontiere, avec lequel il est jumele depuis 1972.</obo:IAO_0000115>
        <oboInOwl:hasOBONamespace>GAZ</oboInOwl:hasOBONamespace>
        <oboInOwl:id>GAZ:00060508</oboInOwl:id>
        <rdfs:label>Parc national de la Vanoise</rdfs:label>
    </owl:NamedIndividual>
    


    <!-- http://purl.obolibrary.org/obo/GAZ_00060509 -->

    <owl:NamedIndividual rdf:about="http://purl.obolibrary.org/obo/GAZ_00060509">
        <obo:RO_0001025 rdf:resource="http://purl.obolibrary.org/obo/GAZ_00060500"/>
        <obo:IAO_0000115>A lake at the Col de la Vanoise.</obo:IAO_0000115>
        <oboInOwl:hasOBONamespace>GAZ</oboInOwl:hasOBONamespace>
        <oboInOwl:id>GAZ:00060509</oboInOwl:id>
        <rdfs:label>Lac Long</rdfs:label>
    </owl:NamedIndividual>
    


    <!-- http://purl.obolibrary.org/obo/GAZ_00060510 -->

    <owl:NamedIndividual rdf:about="http://purl.obolibrary.org/obo/GAZ_00060510">
        <obo:RO_0001025 rdf:resource="http://purl.obolibrary.org/obo/GAZ_00060500"/>
        <obo:IAO_0000115>A lake in the Masiff de Vanoise.</obo:IAO_0000115>
        <oboInOwl:hasOBONamespace>GAZ</oboInOwl:hasOBONamespace>
        <oboInOwl:id>GAZ:00060510</oboInOwl:id>
        <rdfs:label>Lac du Plan-d&apos;Amont</rdfs:label>
    </owl:NamedIndividual>
    


    <!-- http://purl.obolibrary.org/obo/GAZ_00060511 -->

    <owl:NamedIndividual rdf:about="http://purl.obolibrary.org/obo/GAZ_00060511">
        <obo:RO_0001025 rdf:resource="http://purl.obolibrary.org/obo/GAZ_00060500"/>
        <obo:IAO_0000115>A lake in the Masiff de Vanoise.</obo:IAO_0000115>
        <oboInOwl:hasOBONamespace>GAZ</oboInOwl:hasOBONamespace>
        <oboInOwl:id>GAZ:00060511</oboInOwl:id>
        <rdfs:label>Lac du Mont-Coua</rdfs:label>
    </owl:NamedIndividual>
    


    <!-- http://purl.obolibrary.org/obo/GAZ_00060512 -->

    <owl:NamedIndividual rdf:about="http://purl.obolibrary.org/obo/GAZ_00060512">
        <obo:RO_0001025 rdf:resource="http://purl.obolibrary.org/obo/GAZ_00060500"/>
        <obo:IAO_0000115>A lake in the Masiff de Vanoise.</obo:IAO_0000115>
        <oboInOwl:hasOBONamespace>GAZ</oboInOwl:hasOBONamespace>
        <oboInOwl:id>GAZ:00060512</oboInOwl:id>
        <rdfs:label>Lac de la Partie</rdfs:label>
    </owl:NamedIndividual>
    


    <!-- http://purl.obolibrary.org/obo/GAZ_00060513 -->

    <owl:NamedIndividual rdf:about="http://purl.obolibrary.org/obo/GAZ_00060513">
        <obo:RO_0001025 rdf:resource="http://purl.obolibrary.org/obo/GAZ_00060500"/>
        <obo:IAO_0000115>A lake in the Masiff de Vanoise.</obo:IAO_0000115>
        <oboInOwl:hasOBONamespace>GAZ</oboInOwl:hasOBONamespace>
        <oboInOwl:id>GAZ:00060513</oboInOwl:id>
        <rdfs:label>Lac du Lait</rdfs:label>
    </owl:NamedIndividual>
    


    <!-- http://purl.obolibrary.org/obo/GAZ_00060514 -->

    <owl:NamedIndividual rdf:about="http://purl.obolibrary.org/obo/GAZ_00060514">
        <obo:RO_0001025 rdf:resource="http://purl.obolibrary.org/obo/GAZ_00060500"/>
        <obo:IAO_0000115>A lake of glacial origin.</obo:IAO_0000115>
        <oboInOwl:hasOBONamespace>GAZ</oboInOwl:hasOBONamespace>
        <oboInOwl:id>GAZ:00060514</oboInOwl:id>
        <rdfs:label>Lac des Evettes</rdfs:label>
    </owl:NamedIndividual>
    


    <!-- http://purl.obolibrary.org/obo/GAZ_00060515 -->

    <owl:NamedIndividual rdf:about="http://purl.obolibrary.org/obo/GAZ_00060515">
        <obo:RO_0001025 rdf:resource="http://purl.obolibrary.org/obo/GAZ_00060500"/>
        <obo:IAO_0000115>Lakes in the Masiff de Vanoise.</obo:IAO_0000115>
        <oboInOwl:hasOBONamespace>GAZ</oboInOwl:hasOBONamespace>
        <oboInOwl:id>GAZ:00060515</oboInOwl:id>
        <rdfs:label>Lacs de la Roche-Ferran</rdfs:label>
    </owl:NamedIndividual>
    


    <!-- http://purl.obolibrary.org/obo/GAZ_00060516 -->

    <owl:NamedIndividual rdf:about="http://purl.obolibrary.org/obo/GAZ_00060516">
        <obo:RO_0001025 rdf:resource="http://purl.obolibrary.org/obo/GAZ_00060500"/>
        <obo:IAO_0000115>A lake in the Masiff de Vanoise.</obo:IAO_0000115>
        <oboInOwl:hasOBONamespace>GAZ</oboInOwl:hasOBONamespace>
        <oboInOwl:id>GAZ:00060516</oboInOwl:id>
        <rdfs:label>Lac du Plan-du-Lac</rdfs:label>
    </owl:NamedIndividual>
    


    <!-- http://purl.obolibrary.org/obo/GAZ_00060517 -->

    <owl:NamedIndividual rdf:about="http://purl.obolibrary.org/obo/GAZ_00060517">
        <obo:RO_0001025 rdf:resource="http://purl.obolibrary.org/obo/GAZ_00060500"/>
        <obo:IAO_0000115>A lake at the Col de la Vanoise.</obo:IAO_0000115>
        <oboInOwl:hasOBONamespace>GAZ</oboInOwl:hasOBONamespace>
        <oboInOwl:id>GAZ:00060517</oboInOwl:id>
        <rdfs:label>Lac Rond</rdfs:label>
    </owl:NamedIndividual>
    


    <!-- http://purl.obolibrary.org/obo/GAZ_00060518 -->

    <owl:NamedIndividual rdf:about="http://purl.obolibrary.org/obo/GAZ_00060518">
        <obo:RO_0001025 rdf:resource="http://purl.obolibrary.org/obo/GAZ_00060500"/>
        <obo:IAO_0000115>A lake in the Masiff de Vanoise.</obo:IAO_0000115>
        <oboInOwl:hasOBONamespace>GAZ</oboInOwl:hasOBONamespace>
        <oboInOwl:id>GAZ:00060518</oboInOwl:id>
        <rdfs:label>Lac de Toeda</rdfs:label>
    </owl:NamedIndividual>
    


    <!-- http://purl.obolibrary.org/obo/GAZ_00060519 -->

    <owl:NamedIndividual rdf:about="http://purl.obolibrary.org/obo/GAZ_00060519">
        <obo:RO_0001025 rdf:resource="http://purl.obolibrary.org/obo/GAZ_00060500"/>
        <obo:IAO_0000115>A lake in the Masiff de Vanoise.</obo:IAO_0000115>
        <oboInOwl:hasOBONamespace>GAZ</oboInOwl:hasOBONamespace>
        <oboInOwl:id>GAZ:00060519</oboInOwl:id>
        <rdfs:label>Lac du Plan-d&apos;Aval</rdfs:label>
    </owl:NamedIndividual>
    


    <!-- http://purl.obolibrary.org/obo/GAZ_00060520 -->

    <owl:NamedIndividual rdf:about="http://purl.obolibrary.org/obo/GAZ_00060520">
        <obo:RO_0001025 rdf:resource="http://purl.obolibrary.org/obo/GAZ_00060500"/>
        <obo:IAO_0000115>Un lac sur la commune de Val-d&apos;Isere, pres du parc de la Vanoise.</obo:IAO_0000115>
        <oboInOwl:hasOBONamespace>GAZ</oboInOwl:hasOBONamespace>
        <oboInOwl:id>GAZ:00060520</oboInOwl:id>
        <rdfs:label>Lac de la Bailletta</rdfs:label>
    </owl:NamedIndividual>
    


    <!-- http://purl.obolibrary.org/obo/GAZ_00060529 -->

    <owl:NamedIndividual rdf:about="http://purl.obolibrary.org/obo/GAZ_00060529">
        <obo:RO_0001025 rdf:resource="http://purl.obolibrary.org/obo/GAZ_00008200"/>
        <obo:IAO_0000115>A massif and pass (el. 2081 m) in Savoy in France which forms the limit between the Cottian and Graian Alps.</obo:IAO_0000115>
        <oboInOwl:hasOBONamespace>GAZ</oboInOwl:hasOBONamespace>
        <oboInOwl:id>GAZ:00060529</oboInOwl:id>
        <rdfs:label>Massif du Mont Cenis</rdfs:label>
    </owl:NamedIndividual>
    


    <!-- http://purl.obolibrary.org/obo/GAZ_00060530 -->

    <owl:NamedIndividual rdf:about="http://purl.obolibrary.org/obo/GAZ_00060530">
        <obo:RO_0001025 rdf:resource="http://purl.obolibrary.org/obo/GAZ_00060529"/>
        <obo:IAO_0000115>A lake in the Massif du Mont-Cenis.</obo:IAO_0000115>
        <oboInOwl:hasOBONamespace>GAZ</oboInOwl:hasOBONamespace>
        <oboInOwl:id>GAZ:00060530</oboInOwl:id>
        <rdfs:label>Lac Blanc</rdfs:label>
    </owl:NamedIndividual>
    


    <!-- http://purl.obolibrary.org/obo/GAZ_00060531 -->

    <owl:NamedIndividual rdf:about="http://purl.obolibrary.org/obo/GAZ_00060531">
        <obo:RO_0001025 rdf:resource="http://purl.obolibrary.org/obo/GAZ_00060529"/>
        <obo:IAO_0000115>A lake in the Massif du Mont-Cenis.</obo:IAO_0000115>
        <oboInOwl:hasOBONamespace>GAZ</oboInOwl:hasOBONamespace>
        <oboInOwl:id>GAZ:00060531</oboInOwl:id>
        <rdfs:label>Lac du Mont-Cenis</rdfs:label>
    </owl:NamedIndividual>
    


    <!-- http://purl.obolibrary.org/obo/GAZ_00060532 -->

    <owl:NamedIndividual rdf:about="http://purl.obolibrary.org/obo/GAZ_00060532">
        <obo:RO_0001025 rdf:resource="http://purl.obolibrary.org/obo/GAZ_00060529"/>
        <obo:IAO_0000115>A lake in the Massif du Mont-Cenis.</obo:IAO_0000115>
        <oboInOwl:hasOBONamespace>GAZ</oboInOwl:hasOBONamespace>
        <oboInOwl:id>GAZ:00060532</oboInOwl:id>
        <rdfs:label>Lac de Savine</rdfs:label>
    </owl:NamedIndividual>
    


    <!-- http://purl.obolibrary.org/obo/GAZ_00060535 -->

    <owl:NamedIndividual rdf:about="http://purl.obolibrary.org/obo/GAZ_00060535">
        <obo:RO_0001025 rdf:resource="http://purl.obolibrary.org/obo/GAZ_00060182"/>
        <obo:IAO_0000115>A lake in the Massif des Cerces, in Savoie.</obo:IAO_0000115>
        <oboInOwl:hasOBONamespace>GAZ</oboInOwl:hasOBONamespace>
        <oboInOwl:id>GAZ:00060535</oboInOwl:id>
        <rdfs:label>Lac des Cerces</rdfs:label>
    </owl:NamedIndividual>
    


    <!-- http://purl.obolibrary.org/obo/GAZ_00060536 -->

    <owl:NamedIndividual rdf:about="http://purl.obolibrary.org/obo/GAZ_00060536">
        <obo:RO_0001025 rdf:resource="http://purl.obolibrary.org/obo/GAZ_00060182"/>
        <obo:IAO_0000115>A lake in the Massif des Cerces, in Savoie.</obo:IAO_0000115>
        <oboInOwl:hasOBONamespace>GAZ</oboInOwl:hasOBONamespace>
        <oboInOwl:id>GAZ:00060536</oboInOwl:id>
        <rdfs:label>Lac Blanc</rdfs:label>
    </owl:NamedIndividual>
    


    <!-- http://purl.obolibrary.org/obo/GAZ_00060537 -->

    <owl:NamedIndividual rdf:about="http://purl.obolibrary.org/obo/GAZ_00060537">
        <obo:RO_0001025 rdf:resource="http://purl.obolibrary.org/obo/GAZ_00060182"/>
        <obo:IAO_0000115>A lake in the Massif des Cerces, in Savoie.</obo:IAO_0000115>
        <oboInOwl:hasOBONamespace>GAZ</oboInOwl:hasOBONamespace>
        <oboInOwl:id>GAZ:00060537</oboInOwl:id>
        <rdfs:label>Lac Rond</rdfs:label>
    </owl:NamedIndividual>
    


    <!-- http://purl.obolibrary.org/obo/GAZ_00060538 -->

    <owl:NamedIndividual rdf:about="http://purl.obolibrary.org/obo/GAZ_00060538">
        <obo:RO_0001025 rdf:resource="http://purl.obolibrary.org/obo/GAZ_00059214"/>
        <obo:IAO_0000115>A lake in the Grandes Rousses, in Savoie.</obo:IAO_0000115>
        <oboInOwl:hasOBONamespace>GAZ</oboInOwl:hasOBONamespace>
        <oboInOwl:id>GAZ:00060538</oboInOwl:id>
        <rdfs:label>Lac Blanc</rdfs:label>
    </owl:NamedIndividual>
    


    <!-- http://purl.obolibrary.org/obo/GAZ_00060550 -->

    <owl:NamedIndividual rdf:about="http://purl.obolibrary.org/obo/GAZ_00060550">
        <obo:RO_0001025 rdf:resource="http://purl.obolibrary.org/obo/GAZ_00060500"/>
        <obo:IAO_0000115>A glacier.</obo:IAO_0000115>
        <oboInOwl:hasOBONamespace>GAZ</oboInOwl:hasOBONamespace>
        <oboInOwl:id>GAZ:00060550</oboInOwl:id>
        <rdfs:label>Glacier du Pelve</rdfs:label>
    </owl:NamedIndividual>
    


    <!-- http://purl.obolibrary.org/obo/GAZ_00060551 -->

    <owl:NamedIndividual rdf:about="http://purl.obolibrary.org/obo/GAZ_00060551">
        <obo:RO_0001025 rdf:resource="http://purl.obolibrary.org/obo/GAZ_00060500"/>
        <obo:IAO_0000115>A lake associated with the Glacier du Pelve.</obo:IAO_0000115>
        <oboInOwl:hasOBONamespace>GAZ</oboInOwl:hasOBONamespace>
        <oboInOwl:id>GAZ:00060551</oboInOwl:id>
        <rdfs:label>Lac du Pelve</rdfs:label>
    </owl:NamedIndividual>
    


    <!-- http://purl.obolibrary.org/obo/GAZ_00060575 -->

    <owl:NamedIndividual rdf:about="http://purl.obolibrary.org/obo/GAZ_00060575">
        <obo:RO_0001025 rdf:resource="http://purl.obolibrary.org/obo/GAZ_00008197"/>
        <obo:IAO_0000115>A national park in north-west Italy.</obo:IAO_0000115>
        <oboInOwl:hasOBONamespace>GAZ</oboInOwl:hasOBONamespace>
        <oboInOwl:id>GAZ:00060575</oboInOwl:id>
        <rdfs:label>Parco Nazionale del Gran Paradiso</rdfs:label>
    </owl:NamedIndividual>
    


    <!-- http://purl.obolibrary.org/obo/GAZ_00060576 -->

    <owl:NamedIndividual rdf:about="http://purl.obolibrary.org/obo/GAZ_00060576">
        <obo:RO_0001025 rdf:resource="http://purl.obolibrary.org/obo/GAZ_00051917"/>
        <oboInOwl:hasOBONamespace>GAZ</oboInOwl:hasOBONamespace>
        <oboInOwl:id>GAZ:00060576</oboInOwl:id>
        <rdfs:label>Prealps of the Savoie</rdfs:label>
    </owl:NamedIndividual>
    


    <!-- http://purl.obolibrary.org/obo/GAZ_00060577 -->

    <owl:NamedIndividual rdf:about="http://purl.obolibrary.org/obo/GAZ_00060577">
        <obo:RO_0001025 rdf:resource="http://purl.obolibrary.org/obo/GAZ_00060576"/>
        <obo:IAO_0000115>Un massif montagneux des Alpes francaises du nord.</obo:IAO_0000115>
        <oboInOwl:hasOBONamespace>GAZ</oboInOwl:hasOBONamespace>
        <oboInOwl:id>GAZ:00060577</oboInOwl:id>
        <rdfs:label>Massif des Aiguilles Rouges</rdfs:label>
    </owl:NamedIndividual>
    


    <!-- http://purl.obolibrary.org/obo/GAZ_00060578 -->

    <owl:NamedIndividual rdf:about="http://purl.obolibrary.org/obo/GAZ_00060578">
        <obo:RO_0001025 rdf:resource="http://purl.obolibrary.org/obo/GAZ_00060576"/>
        <obo:IAO_0000115>Un massif montagneux des Alpes francaises du nord et suisses.</obo:IAO_0000115>
        <oboInOwl:hasOBONamespace>GAZ</oboInOwl:hasOBONamespace>
        <oboInOwl:id>GAZ:00060578</oboInOwl:id>
        <rdfs:label>Massif du Giffre</rdfs:label>
    </owl:NamedIndividual>
    


    <!-- http://purl.obolibrary.org/obo/GAZ_00060579 -->

    <owl:NamedIndividual rdf:about="http://purl.obolibrary.org/obo/GAZ_00060579">
        <obo:RO_0001025 rdf:resource="http://purl.obolibrary.org/obo/GAZ_00060576"/>
        <obo:IAO_0000115>Un chainon subalpin situe aux trois quarts en Isere et au quart en Savoie. Il s&apos;eleve entre Grenoble (au sud), Chambery (au nord), Voiron et Saint-Laurent-du-Pont (a l&apos;ouest) et le Gresivaudan (vallee de l&apos;Isere, e l&apos;est). Il est borde par le massif du Vercors et la plaine de l&apos;Isere a l&apos;ouest et au sud-ouest, la chaine de Belledonne et la vallee du Gresivaudan au sud-est et a l&apos;est, et le massif des Bauges au nord-est. Il jouxte egalement, au nord-ouest, la chaine de l&apos;Epine.</obo:IAO_0000115>
        <oboInOwl:hasOBONamespace>GAZ</oboInOwl:hasOBONamespace>
        <oboInOwl:id>GAZ:00060579</oboInOwl:id>
        <rdfs:label>Massif de la Chartreuse</rdfs:label>
    </owl:NamedIndividual>
    


    <!-- http://purl.obolibrary.org/obo/GAZ_00060580 -->

    <owl:NamedIndividual rdf:about="http://purl.obolibrary.org/obo/GAZ_00060580">
        <obo:RO_0001025 rdf:resource="http://purl.obolibrary.org/obo/GAZ_00060576"/>
        <obo:IAO_0000115>Un massif montagneux des Prealpes du Nord dans le departement de la Haute-Savoie. Il est limite a l&apos;est par la depression de Thones et la chaine des Aravis.</obo:IAO_0000115>
        <oboInOwl:hasOBONamespace>GAZ</oboInOwl:hasOBONamespace>
        <oboInOwl:id>GAZ:00060580</oboInOwl:id>
        <rdfs:label>Massif des Bornes</rdfs:label>
    </owl:NamedIndividual>
    


    <!-- http://purl.obolibrary.org/obo/GAZ_00060581 -->

    <owl:NamedIndividual rdf:about="http://purl.obolibrary.org/obo/GAZ_00060581">
        <obo:RO_0001025 rdf:resource="http://purl.obolibrary.org/obo/GAZ_00060576"/>
        <obo:IAO_0000115>Un massif situe en Haute-Savoie dans le Chablais francais, et en petite partie dans le canton du Valais (Suisse). Le Massif du Chablais s&apos;etend du Nord au Sud, du Lac Leman a la vallee du Giffre. Il est entoure des Alpes bernoises de l&apos;autre cote du Rhone, du massif du Haut-Giffre au sud-est, et du massif des Bornes au sud de l&apos;Arve.</obo:IAO_0000115>
        <oboInOwl:hasOBONamespace>GAZ</oboInOwl:hasOBONamespace>
        <oboInOwl:id>GAZ:00060581</oboInOwl:id>
        <rdfs:label>Massif du Chablais</rdfs:label>
    </owl:NamedIndividual>
    


    <!-- http://purl.obolibrary.org/obo/GAZ_00060582 -->

    <owl:NamedIndividual rdf:about="http://purl.obolibrary.org/obo/GAZ_00060582">
        <obo:RO_0001025 rdf:resource="http://purl.obolibrary.org/obo/GAZ_00060576"/>
        <obo:IAO_0000115>Un massif montagneux calcaire des prealpes francaises du Nord, se situent a cheval sur les departements de la Savoie et de la Haute-Savoie.</obo:IAO_0000115>
        <oboInOwl:hasOBONamespace>GAZ</oboInOwl:hasOBONamespace>
        <oboInOwl:id>GAZ:00060582</oboInOwl:id>
        <rdfs:label>Massif des Bauges</rdfs:label>
    </owl:NamedIndividual>
    


    <!-- http://purl.obolibrary.org/obo/GAZ_00060583 -->

    <owl:NamedIndividual rdf:about="http://purl.obolibrary.org/obo/GAZ_00060583">
        <obo:RO_0001025 rdf:resource="http://purl.obolibrary.org/obo/GAZ_00060576"/>
        <obo:IAO_0000115>Une chaine de montagnes situee dans les prealpes de Haute-Savoie, et en petite partie en Savoie. Elle s&apos;etend du Nord au Sud, de Cluses a Ugine. A l&apos;ouest, la depression de Thones et le massif des Bornes, au nord-est la vallee de l&apos;Arve et le massif du Haut-Giffre, et au sud-est le val d&apos;Arly (Megeve) et le massif du Beaufortain.</obo:IAO_0000115>
        <oboInOwl:hasOBONamespace>GAZ</oboInOwl:hasOBONamespace>
        <oboInOwl:id>GAZ:00060583</oboInOwl:id>
        <rdfs:label>Chaine des Aravis</rdfs:label>
    </owl:NamedIndividual>
    


    <!-- http://purl.obolibrary.org/obo/GAZ_00060584 -->

    <owl:NamedIndividual rdf:about="http://purl.obolibrary.org/obo/GAZ_00060584">
        <obo:RO_0001025 rdf:resource="http://purl.obolibrary.org/obo/GAZ_00008200"/>
        <obo:IAO_0000115>Un massif montagneux des Alpes franco-italiennes. Il est situe en grande partie sur le departement francais de la Haute-Savoie, mais aussi de la Savoie, sur le val d&apos;Aoste italien et le Valais suisse.</obo:IAO_0000115>
        <oboInOwl:hasOBONamespace>GAZ</oboInOwl:hasOBONamespace>
        <oboInOwl:id>GAZ:00060584</oboInOwl:id>
        <rdfs:label>Massif du Mont-Blanc</rdfs:label>
    </owl:NamedIndividual>
    


    <!-- http://purl.obolibrary.org/obo/GAZ_00060585 -->

    <owl:NamedIndividual rdf:about="http://purl.obolibrary.org/obo/GAZ_00060585">
        <obo:RO_0001025 rdf:resource="http://purl.obolibrary.org/obo/GAZ_00008200"/>
        <obo:IAO_0000115>Un massif des Alpes situe a cheval sur les deux departements de Savoie. Il est limite par l&apos;Isere (vallee de la Tarentaise) au sud, l&apos;Arly au nord-ouest et le Bon-Nant au nord-est. Il est egalement parcouru par la riviere Dorinet puis Doron de Beaufort du nord-est au sud-ouest, au niveau de Beaufort, et leurs affluents, ce qui compartimente quelque peu le massif. Il est entoure des massifs des Aravis, des Bauges, de la Vanoise et du Mont-Blanc.</obo:IAO_0000115>
        <oboInOwl:hasOBONamespace>GAZ</oboInOwl:hasOBONamespace>
        <oboInOwl:id>GAZ:00060585</oboInOwl:id>
        <rdfs:label>Massif du Beaufortain</rdfs:label>
    </owl:NamedIndividual>
    


    <!-- http://purl.obolibrary.org/obo/GAZ_00060586 -->

    <owl:NamedIndividual rdf:about="http://purl.obolibrary.org/obo/GAZ_00060586">
        <obo:RO_0001025 rdf:resource="http://purl.obolibrary.org/obo/GAZ_00008200"/>
        <obo:IAO_0000115>Un massif des Alpes franaises qui se situe en Savoie entre la rive droite de la Basse-Maurienne et la rive gauche de la vallee de la Tarentaise.</obo:IAO_0000115>
        <oboInOwl:hasOBONamespace>GAZ</oboInOwl:hasOBONamespace>
        <oboInOwl:id>GAZ:00060586</oboInOwl:id>
        <rdfs:label>Massif de la Lauziere</rdfs:label>
    </owl:NamedIndividual>
    


    <!-- http://purl.obolibrary.org/obo/GAZ_00060587 -->

    <owl:NamedIndividual rdf:about="http://purl.obolibrary.org/obo/GAZ_00060587">
        <obo:RO_0001025 rdf:resource="http://purl.obolibrary.org/obo/GAZ_00009675"/>
        <obo:IAO_0000115>Un massif des Alpes francaises situe sur les departements de la Savoie, de l&apos;Isere et des Hautes-Alpes. L&apos;Oisans couvre une partie du massif.</obo:IAO_0000115>
        <oboInOwl:hasOBONamespace>GAZ</oboInOwl:hasOBONamespace>
        <oboInOwl:id>GAZ:00060587</oboInOwl:id>
        <rdfs:label>Massif d&apos;Arvan-Villards</rdfs:label>
    </owl:NamedIndividual>
    


    <!-- http://purl.obolibrary.org/obo/GAZ_00060588 -->

    <owl:NamedIndividual rdf:about="http://purl.obolibrary.org/obo/GAZ_00060588">
        <obo:RO_0001025 rdf:resource="http://purl.obolibrary.org/obo/GAZ_00008405"/>
        <obo:IAO_0000115>Un massif des Alpes du Nord a la frontiere entre la France (departement de la Savoie) et l&apos;Italie.</obo:IAO_0000115>
        <oboInOwl:hasOBONamespace>GAZ</oboInOwl:hasOBONamespace>
        <oboInOwl:id>GAZ:00060588</oboInOwl:id>
        <rdfs:label>Massif du Mont-Cenis</rdfs:label>
    </owl:NamedIndividual>
    


    <!-- http://purl.obolibrary.org/obo/GAZ_00060589 -->

    <owl:NamedIndividual rdf:about="http://purl.obolibrary.org/obo/GAZ_00060589">
        <obo:RO_0001025 rdf:resource="http://purl.obolibrary.org/obo/GAZ_00008405"/>
        <obo:IAO_0000115>Un massif des Alpes franco-italiennes situe sur les departements des Hautes-Alpes et des Alpes-de-Haute-Provence, ainsi que dans la region Piemont.</obo:IAO_0000115>
        <oboInOwl:hasOBONamespace>GAZ</oboInOwl:hasOBONamespace>
        <oboInOwl:id>GAZ:00060589</oboInOwl:id>
        <rdfs:label>Massif de l&apos;Ubaye</rdfs:label>
    </owl:NamedIndividual>
    


    <!-- http://purl.obolibrary.org/obo/GAZ_00060590 -->

    <owl:NamedIndividual rdf:about="http://purl.obolibrary.org/obo/GAZ_00060590">
        <obo:RO_0001025 rdf:resource="http://purl.obolibrary.org/obo/GAZ_00051917"/>
        <oboInOwl:hasOBONamespace>GAZ</oboInOwl:hasOBONamespace>
        <oboInOwl:id>GAZ:00060590</oboInOwl:id>
        <rdfs:label>Dauphine Prealps</rdfs:label>
    </owl:NamedIndividual>
    


    <!-- http://purl.obolibrary.org/obo/GAZ_00060591 -->

    <owl:NamedIndividual rdf:about="http://purl.obolibrary.org/obo/GAZ_00060591">
        <obo:RO_0001025 rdf:resource="http://purl.obolibrary.org/obo/GAZ_00060590"/>
        <obo:IAO_0000115>A mountain massif. It lies west of the Dauphine Alps, from which it is separated by the rivers Drac and Isere. Cliffs at its eastern edge face the city of Grenoble.</obo:IAO_0000115>
        <oboInOwl:hasOBONamespace>GAZ</oboInOwl:hasOBONamespace>
        <oboInOwl:id>GAZ:00060591</oboInOwl:id>
        <rdfs:label>Massif du Vercors</rdfs:label>
    </owl:NamedIndividual>
    


    <!-- http://purl.obolibrary.org/obo/GAZ_00060592 -->

    <owl:NamedIndividual rdf:about="http://purl.obolibrary.org/obo/GAZ_00060592">
        <obo:RO_0001025 rdf:resource="http://purl.obolibrary.org/obo/GAZ_00060590"/>
        <oboInOwl:hasOBONamespace>GAZ</oboInOwl:hasOBONamespace>
        <oboInOwl:id>GAZ:00060592</oboInOwl:id>
        <rdfs:label>Massif du Diois</rdfs:label>
    </owl:NamedIndividual>
    


    <!-- http://purl.obolibrary.org/obo/GAZ_00060593 -->

    <owl:NamedIndividual rdf:about="http://purl.obolibrary.org/obo/GAZ_00060593">
        <obo:RO_0001025 rdf:resource="http://purl.obolibrary.org/obo/GAZ_00060590"/>
        <oboInOwl:hasOBONamespace>GAZ</oboInOwl:hasOBONamespace>
        <oboInOwl:id>GAZ:00060593</oboInOwl:id>
        <rdfs:label>Massif des Baronnies</rdfs:label>
    </owl:NamedIndividual>
    


    <!-- http://purl.obolibrary.org/obo/GAZ_00060594 -->

    <owl:NamedIndividual rdf:about="http://purl.obolibrary.org/obo/GAZ_00060594">
        <obo:RO_0001025 rdf:resource="http://purl.obolibrary.org/obo/GAZ_00060590"/>
        <oboInOwl:hasOBONamespace>GAZ</oboInOwl:hasOBONamespace>
        <oboInOwl:id>GAZ:00060594</oboInOwl:id>
        <rdfs:label>Bochaine</rdfs:label>
    </owl:NamedIndividual>
    


    <!-- http://purl.obolibrary.org/obo/GAZ_00060595 -->

    <owl:NamedIndividual rdf:about="http://purl.obolibrary.org/obo/GAZ_00060595">
        <obo:RO_0001025 rdf:resource="http://purl.obolibrary.org/obo/GAZ_00060590"/>
        <obo:IAO_0000115>A mountain range of the French Prealps located in the departement of Vaucluse, between the Luberon Massif and Mont Ventoux.</obo:IAO_0000115>
        <oboInOwl:hasOBONamespace>GAZ</oboInOwl:hasOBONamespace>
        <oboInOwl:id>GAZ:00060595</oboInOwl:id>
        <rdfs:label>Monts de Vaucluse</rdfs:label>
    </owl:NamedIndividual>
    


    <!-- http://purl.obolibrary.org/obo/GAZ_00060596 -->

    <owl:NamedIndividual rdf:about="http://purl.obolibrary.org/obo/GAZ_00060596">
        <obo:RO_0001025 rdf:resource="http://purl.obolibrary.org/obo/GAZ_00060590"/>
        <obo:IAO_0000115>A mountain massif.</obo:IAO_0000115>
        <oboInOwl:hasOBONamespace>GAZ</oboInOwl:hasOBONamespace>
        <oboInOwl:id>GAZ:00060596</oboInOwl:id>
        <rdfs:label>Massif du Devoluy</rdfs:label>
    </owl:NamedIndividual>
    


    <!-- http://purl.obolibrary.org/obo/GAZ_00060597 -->

    <owl:NamedIndividual rdf:about="http://purl.obolibrary.org/obo/GAZ_00060597">
        <obo:RO_0001025 rdf:resource="http://purl.obolibrary.org/obo/GAZ_00051917"/>
        <oboInOwl:hasOBONamespace>GAZ</oboInOwl:hasOBONamespace>
        <oboInOwl:id>GAZ:00060597</oboInOwl:id>
        <rdfs:label>Alpes de Provence</rdfs:label>
    </owl:NamedIndividual>
    


    <!-- http://purl.obolibrary.org/obo/GAZ_00060598 -->

    <owl:NamedIndividual rdf:about="http://purl.obolibrary.org/obo/GAZ_00060598">
        <obo:RO_0001025 rdf:resource="http://purl.obolibrary.org/obo/GAZ_00060597"/>
        <oboInOwl:hasOBONamespace>GAZ</oboInOwl:hasOBONamespace>
        <oboInOwl:id>GAZ:00060598</oboInOwl:id>
        <rdfs:label>Prealpes de Castellane</rdfs:label>
    </owl:NamedIndividual>
    


    <!-- http://purl.obolibrary.org/obo/GAZ_00060599 -->

    <owl:NamedIndividual rdf:about="http://purl.obolibrary.org/obo/GAZ_00060599">
        <obo:RO_0001025 rdf:resource="http://purl.obolibrary.org/obo/GAZ_00060597"/>
        <oboInOwl:hasOBONamespace>GAZ</oboInOwl:hasOBONamespace>
        <oboInOwl:id>GAZ:00060599</oboInOwl:id>
        <rdfs:label>Prealpes de Digne</rdfs:label>
    </owl:NamedIndividual>
    


    <!-- http://purl.obolibrary.org/obo/GAZ_00060600 -->

    <owl:NamedIndividual rdf:about="http://purl.obolibrary.org/obo/GAZ_00060600">
        <obo:RO_0001025 rdf:resource="http://purl.obolibrary.org/obo/GAZ_00060597"/>
        <oboInOwl:hasOBONamespace>GAZ</oboInOwl:hasOBONamespace>
        <oboInOwl:id>GAZ:00060600</oboInOwl:id>
        <rdfs:label>Massif des Trois-Eveches</rdfs:label>
    </owl:NamedIndividual>
    


    <!-- http://purl.obolibrary.org/obo/GAZ_00060601 -->

    <owl:NamedIndividual rdf:about="http://purl.obolibrary.org/obo/GAZ_00060601">
        <obo:RO_0001025 rdf:resource="http://purl.obolibrary.org/obo/GAZ_00051917"/>
        <oboInOwl:hasOBONamespace>GAZ</oboInOwl:hasOBONamespace>
        <oboInOwl:id>GAZ:00060601</oboInOwl:id>
        <rdfs:label>Prealpes de Provence</rdfs:label>
    </owl:NamedIndividual>
    


    <!-- http://purl.obolibrary.org/obo/GAZ_00060602 -->

    <owl:NamedIndividual rdf:about="http://purl.obolibrary.org/obo/GAZ_00060602">
        <obo:RO_0001025 rdf:resource="http://purl.obolibrary.org/obo/GAZ_00009679"/>
        <oboInOwl:hasOBONamespace>GAZ</oboInOwl:hasOBONamespace>
        <oboInOwl:id>GAZ:00060602</oboInOwl:id>
        <rdfs:label>Massif du Pelat</rdfs:label>
    </owl:NamedIndividual>
    


    <!-- http://purl.obolibrary.org/obo/GAZ_00060603 -->

    <owl:NamedIndividual rdf:about="http://purl.obolibrary.org/obo/GAZ_00060603">
        <obo:RO_0001025 rdf:resource="http://purl.obolibrary.org/obo/GAZ_00060601"/>
        <oboInOwl:hasOBONamespace>GAZ</oboInOwl:hasOBONamespace>
        <oboInOwl:id>GAZ:00060603</oboInOwl:id>
        <rdfs:label>Massif de l&apos;Etoile</rdfs:label>
    </owl:NamedIndividual>
    


    <!-- http://purl.obolibrary.org/obo/GAZ_00060604 -->

    <owl:NamedIndividual rdf:about="http://purl.obolibrary.org/obo/GAZ_00060604">
        <obo:RO_0001025 rdf:resource="http://purl.obolibrary.org/obo/GAZ_00060597"/>
        <obo:RO_0001025 rdf:resource="http://purl.obolibrary.org/obo/GAZ_00060601"/>
        <oboInOwl:hasOBONamespace>GAZ</oboInOwl:hasOBONamespace>
        <oboInOwl:id>GAZ:00060604</oboInOwl:id>
        <rdfs:label>Montagne Sainte-Victoire</rdfs:label>
    </owl:NamedIndividual>
    


    <!-- http://purl.obolibrary.org/obo/GAZ_00060605 -->

    <owl:NamedIndividual rdf:about="http://purl.obolibrary.org/obo/GAZ_00060605">
        <obo:RO_0001025 rdf:resource="http://purl.obolibrary.org/obo/GAZ_00060601"/>
        <oboInOwl:hasOBONamespace>GAZ</oboInOwl:hasOBONamespace>
        <oboInOwl:id>GAZ:00060605</oboInOwl:id>
        <rdfs:label>Massif du Garlaban</rdfs:label>
    </owl:NamedIndividual>
    


    <!-- http://purl.obolibrary.org/obo/GAZ_00060606 -->

    <owl:NamedIndividual rdf:about="http://purl.obolibrary.org/obo/GAZ_00060606">
        <obo:RO_0001025 rdf:resource="http://purl.obolibrary.org/obo/GAZ_00009679"/>
        <oboInOwl:hasOBONamespace>GAZ</oboInOwl:hasOBONamespace>
        <oboInOwl:id>GAZ:00060606</oboInOwl:id>
        <rdfs:label>Prealpes de Grasse</rdfs:label>
    </owl:NamedIndividual>
    


    <!-- http://purl.obolibrary.org/obo/GAZ_00060607 -->

    <owl:NamedIndividual rdf:about="http://purl.obolibrary.org/obo/GAZ_00060607">
        <obo:RO_0001025 rdf:resource="http://purl.obolibrary.org/obo/GAZ_00009679"/>
        <oboInOwl:hasOBONamespace>GAZ</oboInOwl:hasOBONamespace>
        <oboInOwl:id>GAZ:00060607</oboInOwl:id>
        <rdfs:label>Prealpes de Nice</rdfs:label>
    </owl:NamedIndividual>
    


    <!-- http://purl.obolibrary.org/obo/GAZ_00060608 -->

    <owl:NamedIndividual rdf:about="http://purl.obolibrary.org/obo/GAZ_00060608">
        <obo:RO_0001025 rdf:resource="http://purl.obolibrary.org/obo/GAZ_00009679"/>
        <obo:IAO_0000115>Un massif des Alpes situe a cheval sur les departements francais des Alpes-Maritimes et des Alpes-de-Haute-Provence et sur le Piemont italien.</obo:IAO_0000115>
        <oboInOwl:hasOBONamespace>GAZ</oboInOwl:hasOBONamespace>
        <oboInOwl:id>GAZ:00060608</oboInOwl:id>
        <rdfs:label>Massif du Mercantour</rdfs:label>
    </owl:NamedIndividual>
    


    <!-- http://purl.obolibrary.org/obo/GAZ_00060609 -->

    <owl:NamedIndividual rdf:about="http://purl.obolibrary.org/obo/GAZ_00060609">
        <oboInOwl:hasOBONamespace>GAZ</oboInOwl:hasOBONamespace>
        <oboInOwl:id>GAZ:00060609</oboInOwl:id>
        <rdfs:label>Central Alps</rdfs:label>
    </owl:NamedIndividual>
    


    <!-- http://purl.obolibrary.org/obo/GAZ_00060610 -->

    <owl:NamedIndividual rdf:about="http://purl.obolibrary.org/obo/GAZ_00060610">
        <obo:RO_0001025 rdf:resource="http://purl.obolibrary.org/obo/GAZ_00009676"/>
        <oboInOwl:hasOBONamespace>GAZ</oboInOwl:hasOBONamespace>
        <oboInOwl:id>GAZ:00060610</oboInOwl:id>
        <rdfs:label>Prealpes Bernoises</rdfs:label>
    </owl:NamedIndividual>
    


    <!-- http://purl.obolibrary.org/obo/GAZ_00060611 -->

    <owl:NamedIndividual rdf:about="http://purl.obolibrary.org/obo/GAZ_00060611">
        <obo:RO_0001025 rdf:resource="http://purl.obolibrary.org/obo/GAZ_00009676"/>
        <oboInOwl:hasOBONamespace>GAZ</oboInOwl:hasOBONamespace>
        <oboInOwl:id>GAZ:00060611</oboInOwl:id>
        <rdfs:label>Prealpes Fribourgeoises</rdfs:label>
    </owl:NamedIndividual>
    


    <!-- http://purl.obolibrary.org/obo/GAZ_00060614 -->

    <owl:NamedIndividual rdf:about="http://purl.obolibrary.org/obo/GAZ_00060614">
        <obo:RO_0001025 rdf:resource="http://purl.obolibrary.org/obo/GAZ_00008403"/>
        <oboInOwl:hasOBONamespace>GAZ</oboInOwl:hasOBONamespace>
        <oboInOwl:id>GAZ:00060614</oboInOwl:id>
        <rdfs:label>Prealpes Biellaises</rdfs:label>
    </owl:NamedIndividual>
    


    <!-- http://purl.obolibrary.org/obo/GAZ_00060615 -->

    <owl:NamedIndividual rdf:about="http://purl.obolibrary.org/obo/GAZ_00060615">
        <obo:RO_0001025 rdf:resource="http://purl.obolibrary.org/obo/GAZ_00056810"/>
        <oboInOwl:hasOBONamespace>GAZ</oboInOwl:hasOBONamespace>
        <oboInOwl:id>GAZ:00060615</oboInOwl:id>
        <rdfs:label>Massif du Saint-Gothard</rdfs:label>
    </owl:NamedIndividual>
    


    <!-- http://purl.obolibrary.org/obo/GAZ_00060616 -->

    <owl:NamedIndividual rdf:about="http://purl.obolibrary.org/obo/GAZ_00060616">
        <obo:RO_0001025 rdf:resource="http://purl.obolibrary.org/obo/GAZ_00009680"/>
        <obo:IAO_0000115>Un massif des Alpes lepontines compris entre le col du Saint-Gothard et le col du Splugen, principalement situe sur les cantons des Grisons et du Tessin, mais egalement en Lombardie.</obo:IAO_0000115>
        <oboInOwl:hasOBONamespace>GAZ</oboInOwl:hasOBONamespace>
        <oboInOwl:id>GAZ:00060616</oboInOwl:id>
        <rdfs:label>Adula</rdfs:label>
    </owl:NamedIndividual>
    


    <!-- http://purl.obolibrary.org/obo/GAZ_00060617 -->

    <owl:NamedIndividual rdf:about="http://purl.obolibrary.org/obo/GAZ_00060617">
        <obo:RO_0001025 rdf:resource="http://purl.obolibrary.org/obo/GAZ_00009680"/>
        <oboInOwl:hasOBONamespace>GAZ</oboInOwl:hasOBONamespace>
        <oboInOwl:id>GAZ:00060617</oboInOwl:id>
        <rdfs:label>Alpes Tessinoises</rdfs:label>
    </owl:NamedIndividual>
    


    <!-- http://purl.obolibrary.org/obo/GAZ_00060618 -->

    <owl:NamedIndividual rdf:about="http://purl.obolibrary.org/obo/GAZ_00060618">
        <obo:RO_0001025 rdf:resource="http://purl.obolibrary.org/obo/GAZ_00060617"/>
        <oboInOwl:hasOBONamespace>GAZ</oboInOwl:hasOBONamespace>
        <oboInOwl:id>GAZ:00060618</oboInOwl:id>
        <rdfs:label>Massif du Monte Leone</rdfs:label>
    </owl:NamedIndividual>
    


    <!-- http://purl.obolibrary.org/obo/GAZ_00060619 -->

    <owl:NamedIndividual rdf:about="http://purl.obolibrary.org/obo/GAZ_00060619">
        <obo:RO_0001025 rdf:resource="http://purl.obolibrary.org/obo/GAZ_00060617"/>
        <oboInOwl:hasOBONamespace>GAZ</oboInOwl:hasOBONamespace>
        <oboInOwl:id>GAZ:00060619</oboInOwl:id>
        <rdfs:label>Massif du Saint-Gothard</rdfs:label>
    </owl:NamedIndividual>
    


    <!-- http://purl.obolibrary.org/obo/GAZ_00060620 -->

    <owl:NamedIndividual rdf:about="http://purl.obolibrary.org/obo/GAZ_00060620">
        <obo:RO_0001025 rdf:resource="http://purl.obolibrary.org/obo/GAZ_00060616"/>
        <oboInOwl:hasOBONamespace>GAZ</oboInOwl:hasOBONamespace>
        <oboInOwl:id>GAZ:00060620</oboInOwl:id>
        <rdfs:label>Massif du Ceneri</rdfs:label>
    </owl:NamedIndividual>
    


    <!-- http://purl.obolibrary.org/obo/GAZ_00060621 -->

    <owl:NamedIndividual rdf:about="http://purl.obolibrary.org/obo/GAZ_00060621">
        <obo:RO_0001025 rdf:resource="http://purl.obolibrary.org/obo/GAZ_00060609"/>
        <obo:IAO_0000115>A mountain range in Switzerland on the northern edge of the Alps. They extend into the cantons of Appenzell Ausserrhoden, Appenzell Innerrhoden and St. Gallen and are bordered by the Glarus Alps to the west and the RAtikon to the south-east.</obo:IAO_0000115>
        <oboInOwl:hasOBONamespace>GAZ</oboInOwl:hasOBONamespace>
        <oboInOwl:id>GAZ:00060621</oboInOwl:id>
        <rdfs:label>Appenzell Alps</rdfs:label>
    </owl:NamedIndividual>
    


    <!-- http://purl.obolibrary.org/obo/GAZ_00060622 -->

    <owl:NamedIndividual rdf:about="http://purl.obolibrary.org/obo/GAZ_00060622">
        <obo:RO_0001025 rdf:resource="http://purl.obolibrary.org/obo/GAZ_00051914"/>
        <obo:IAO_0000115>Un ensemble des Alpes orientales centrales compris entre la vallee de l&apos;Inn au nord, la vallee de l&apos;Adige (val venoste) au sud et celle de l&apos;Isarco au sud-est, entre l&apos;Autriche et l&apos;Italie. L&apos;Otztal s&apos;ecoule egalement au sein de cet ensemble, en direction du nord.</obo:IAO_0000115>
        <oboInOwl:hasOBONamespace>GAZ</oboInOwl:hasOBONamespace>
        <oboInOwl:id>GAZ:00060622</oboInOwl:id>
        <rdfs:label>Alpes Atesines</rdfs:label>
    </owl:NamedIndividual>
    


    <!-- http://purl.obolibrary.org/obo/GAZ_00060623 -->

    <owl:NamedIndividual rdf:about="http://purl.obolibrary.org/obo/GAZ_00060623">
        <obo:RO_0001025 rdf:resource="http://purl.obolibrary.org/obo/GAZ_00060622"/>
        <obo:IAO_0000115>Un massif des Alpes orientales centrales. Elles s&apos;elevent en Italie (province de Bolzano), entre les rives de l&apos;Adige et de l&apos;Isarco. Une autre vallee, la vallee de Sarentino ou Sarntal, qui s&apos;ecoule au coeur du massif vers le sud, lui donne son nom. Le massif est entoure des Alpes de Stubai au nord, des Alpes de Zillertal au nord-est, des Dolomites au sud-est, des Alpes de Fiemme au sud, du massif de Non au sud-ouest, du massif de l&apos;Ortles et des Alpes de l&apos;Otztal a l&apos;ouest.</obo:IAO_0000115>
        <oboInOwl:hasOBONamespace>GAZ</oboInOwl:hasOBONamespace>
        <oboInOwl:id>GAZ:00060623</oboInOwl:id>
        <rdfs:label>Sarntal Alps</rdfs:label>
    </owl:NamedIndividual>
    


    <!-- http://purl.obolibrary.org/obo/GAZ_00060624 -->

    <owl:NamedIndividual rdf:about="http://purl.obolibrary.org/obo/GAZ_00060624">
        <obo:RO_0001025 rdf:resource="http://purl.obolibrary.org/obo/GAZ_00051914"/>
        <obo:IAO_0000115>Un ensemble des Alpes orientales centrales compris entre la vallee de l&apos;Inn au nord-ouest, la vallee de l&apos;Enns au nord et celle de la Drave au sud, entre l&apos;Autriche et l&apos;Italie, et plus infimement en Slovenie. La Mur s&apos;ecoule egalement au sein de cet ensemble, en direction de l&apos;est.</obo:IAO_0000115>
        <oboInOwl:hasOBONamespace>GAZ</oboInOwl:hasOBONamespace>
        <oboInOwl:id>GAZ:00060624</oboInOwl:id>
        <rdfs:label>Noric Alps</rdfs:label>
    </owl:NamedIndividual>
    


    <!-- http://purl.obolibrary.org/obo/GAZ_00060625 -->

    <owl:NamedIndividual rdf:about="http://purl.obolibrary.org/obo/GAZ_00060625">
        <obo:RO_0001025 rdf:resource="http://purl.obolibrary.org/obo/GAZ_00051914"/>
        <obo:IAO_0000115>Un massif des Alpes orientales centrales. Elles s&apos;elevent principalement en Autriche (land de Carinthie et land de Styrie) mais egalement en Slovenie.</obo:IAO_0000115>
        <oboInOwl:hasOBONamespace>GAZ</oboInOwl:hasOBONamespace>
        <oboInOwl:id>GAZ:00060625</oboInOwl:id>
        <rdfs:label>Lavanttal Alps</rdfs:label>
    </owl:NamedIndividual>
    


    <!-- http://purl.obolibrary.org/obo/GAZ_00060626 -->

    <owl:NamedIndividual rdf:about="http://purl.obolibrary.org/obo/GAZ_00060626">
        <obo:RO_0001025 rdf:resource="http://purl.obolibrary.org/obo/GAZ_00051914"/>
        <obo:IAO_0000115>Un massif des Alpes orientales centrales. Elles s&apos;elevent en Autriche (principalement land de Carinthie, mais egalement land de Salzbourg et land de Styrie).</obo:IAO_0000115>
        <oboInOwl:hasOBONamespace>GAZ</oboInOwl:hasOBONamespace>
        <oboInOwl:id>GAZ:00060626</oboInOwl:id>
        <rdfs:label>Gurktal Alps</rdfs:label>
    </owl:NamedIndividual>
    


    <!-- http://purl.obolibrary.org/obo/GAZ_00060627 -->

    <owl:NamedIndividual rdf:about="http://purl.obolibrary.org/obo/GAZ_00060627">
        <obo:RO_0001025 rdf:resource="http://purl.obolibrary.org/obo/GAZ_00051914"/>
        <obo:IAO_0000115>Un massif des Alpes orientales centrales. Il s&apos;eleve entre l&apos;Autriche (Tyrol) et la Suisse (canton des Grisons), sur la rive gauche de l&apos;Inn.</obo:IAO_0000115>
        <oboInOwl:hasOBONamespace>GAZ</oboInOwl:hasOBONamespace>
        <oboInOwl:id>GAZ:00060627</oboInOwl:id>
        <rdfs:label>Massif de Samnaun</rdfs:label>
    </owl:NamedIndividual>
    


    <!-- http://purl.obolibrary.org/obo/GAZ_00060628 -->

    <owl:NamedIndividual rdf:about="http://purl.obolibrary.org/obo/GAZ_00060628">
        <obo:RO_0001025 rdf:resource="http://purl.obolibrary.org/obo/GAZ_00051916"/>
        <obo:IAO_0000115>A mountain range, made of metamorphic stones, near to the Southern Limestone Alps in north Slovenia near Dravograd and Maribor.</obo:IAO_0000115>
        <oboInOwl:hasOBONamespace>GAZ</oboInOwl:hasOBONamespace>
        <oboInOwl:id>GAZ:00060628</oboInOwl:id>
        <rdfs:label>Pohorje</rdfs:label>
    </owl:NamedIndividual>
    


    <!-- http://purl.obolibrary.org/obo/GAZ_00060629 -->

    <owl:NamedIndividual rdf:about="http://purl.obolibrary.org/obo/GAZ_00060629">
        <obo:RO_0001025 rdf:resource="http://purl.obolibrary.org/obo/GAZ_00051916"/>
        <obo:IAO_0000115>Un massif des Prealpes orientales meridionales. Elles s&apos;elevent en Italie (Trentin-Haut-Adige). Le massif est entoure des Alpes de Sarntal au nord, du massif des Dolomites e l&apos;est, des Prealpes vicentines au sud et des massifs de Brenta et de Non a l&apos;ouest. Il est borde par l&apos;Adige a l&apos;ouest et la Brenta au sud. Le Val di Fiemme et le Val di Cembra traversent le massif vers le sud-ouest au gre du cours de l&apos;Avisio.</obo:IAO_0000115>
        <oboInOwl:hasOBONamespace>GAZ</oboInOwl:hasOBONamespace>
        <oboInOwl:id>GAZ:00060629</oboInOwl:id>
        <rdfs:label>Alpes de Fiemme</rdfs:label>
    </owl:NamedIndividual>
    


    <!-- http://purl.obolibrary.org/obo/GAZ_00060630 -->

    <owl:NamedIndividual rdf:about="http://purl.obolibrary.org/obo/GAZ_00060630">
        <obo:RO_0001025 rdf:resource="http://purl.obolibrary.org/obo/GAZ_00051916"/>
        <obo:IAO_0000115>Un massif des Prealpes orientales meridionales. Elles s&apos;elevent en Italie (limite entre le Trentin-Haut-Adige et la Venetie), au nord de Vicence.</obo:IAO_0000115>
        <oboInOwl:hasOBONamespace>GAZ</oboInOwl:hasOBONamespace>
        <oboInOwl:id>GAZ:00060630</oboInOwl:id>
        <rdfs:label>Prealpes Vicentines</rdfs:label>
    </owl:NamedIndividual>
    


    <!-- http://purl.obolibrary.org/obo/GAZ_00060631 -->

    <owl:NamedIndividual rdf:about="http://purl.obolibrary.org/obo/GAZ_00060631">
        <obo:RO_0001025 rdf:resource="http://purl.obolibrary.org/obo/GAZ_00051916"/>
        <obo:IAO_0000115>Un massif des Prealpes orientales meridionales. Il s&apos;eleve en Italie (Trentin-Haut-Adige), au sud-ouest de Bolzano. Il est traverse par le Val di Non.</obo:IAO_0000115>
        <oboInOwl:hasOBONamespace>GAZ</oboInOwl:hasOBONamespace>
        <oboInOwl:id>GAZ:00060631</oboInOwl:id>
        <rdfs:label>Massif de Non</rdfs:label>
    </owl:NamedIndividual>
    


    <!-- http://purl.obolibrary.org/obo/GAZ_00060632 -->

    <owl:NamedIndividual rdf:about="http://purl.obolibrary.org/obo/GAZ_00060632">
        <obo:RO_0001025 rdf:resource="http://purl.obolibrary.org/obo/GAZ_00051916"/>
        <obo:IAO_0000115>Un massif des Prealpes orientales meridionales. Elles s&apos;elevent en Italie (limite entre le Trentin-Haut-Adige, la Lombardie et la Venetie). Les montagnes sont orientees nord-sud autour de la cuvette formee par le lac de Garde et sont entourees du massif d&apos;Adamello-Presanella a l&apos;ouest, du massif de Brenta au nord et des Prealpes vicentines a l&apos;est.</obo:IAO_0000115>
        <oboInOwl:hasOBONamespace>GAZ</oboInOwl:hasOBONamespace>
        <oboInOwl:id>GAZ:00060632</oboInOwl:id>
        <rdfs:label>Montagnes autour du lac de Garde</rdfs:label>
    </owl:NamedIndividual>
    


    <!-- http://purl.obolibrary.org/obo/GAZ_00060633 -->

    <owl:NamedIndividual rdf:about="http://purl.obolibrary.org/obo/GAZ_00060633">
        <obo:RO_0001025 rdf:resource="http://purl.obolibrary.org/obo/GAZ_00051916"/>
        <obo:IAO_0000115>Un massif des Prealpes orientales meridionales. Il s&apos;eleve en Italie (Lombardie). Le massif est entoure du massif de l&apos;Ortles au nord-est, du massif de l&apos;Adamello-Presanella au sud-est, des Alpes bergamasques au sud et de la chaine de Livigno au nord-ouest. Il est borde par l&apos;Adda (Valteline) a l&apos;ouest et l&apos;Oglio (Val Camonica) au sud.</obo:IAO_0000115>
        <oboInOwl:hasOBONamespace>GAZ</oboInOwl:hasOBONamespace>
        <oboInOwl:id>GAZ:00060633</oboInOwl:id>
        <rdfs:label>Massif de Sobretta-Gavia</rdfs:label>
    </owl:NamedIndividual>
    


    <!-- http://purl.obolibrary.org/obo/GAZ_00060634 -->

    <owl:NamedIndividual rdf:about="http://purl.obolibrary.org/obo/GAZ_00060634">
        <obo:RO_0001025 rdf:resource="http://purl.obolibrary.org/obo/GAZ_00051915"/>
        <obo:IAO_0000115>Un massif des Prealpes orientales septentrionales. Il s&apos;eleve en Autriche (Basse-Autriche) et tient som nom de Gutenstein, une localite au coeur des montagnes. Le massif est entoure par le Wienerwald au nord, les montagnes a l&apos;est de la Mur a l&apos;est, le massif du Rax et Schneeberg au sud, les Alpes de Murzsteg au sud-ouest et les Alpes de Turnitz a l&apos;ouest.</obo:IAO_0000115>
        <oboInOwl:hasOBONamespace>GAZ</oboInOwl:hasOBONamespace>
        <oboInOwl:id>GAZ:00060634</oboInOwl:id>
        <rdfs:label>Alpes de Gutenstein</rdfs:label>
    </owl:NamedIndividual>
    


    <!-- http://purl.obolibrary.org/obo/GAZ_00060635 -->

    <owl:NamedIndividual rdf:about="http://purl.obolibrary.org/obo/GAZ_00060635">
        <obo:RO_0001025 rdf:resource="http://purl.obolibrary.org/obo/GAZ_00051915"/>
        <obo:IAO_0000115>Un massif des Peealpes orientales septentrionales. Il s&apos;eleve en Autriche (limite entre la Basse-Autriche et le land de Styrie). Le massif est entoure par les Alpes de Gutenstein au nord, les montagnes de la rive gauche de la Mur au sud-est et les Alpes de Murzsteg a l&apos;ouest.</obo:IAO_0000115>
        <oboInOwl:hasOBONamespace>GAZ</oboInOwl:hasOBONamespace>
        <oboInOwl:id>GAZ:00060635</oboInOwl:id>
        <rdfs:label>Rax et Schneeberg</rdfs:label>
    </owl:NamedIndividual>
    


    <!-- http://purl.obolibrary.org/obo/GAZ_00060636 -->

    <owl:NamedIndividual rdf:about="http://purl.obolibrary.org/obo/GAZ_00060636">
        <obo:RO_0001025 rdf:resource="http://purl.obolibrary.org/obo/GAZ_00051915"/>
        <obo:IAO_0000115>Un massif des Prealpes orientales septentrionales. Il s&apos;eleve en Autriche (limite entre la Basse-Autriche et le land de Styrie). Le massif est entoure par les Alpes de Turnitz au nord, les Alpes de Gutenstein au nord-est, Rax et Schneeberg a l&apos;est, les montagnes a l&apos;est de la Mur au sud-est et le massif du Hochschwab a l&apos;ouest.</obo:IAO_0000115>
        <oboInOwl:hasOBONamespace>GAZ</oboInOwl:hasOBONamespace>
        <oboInOwl:id>GAZ:00060636</oboInOwl:id>
        <rdfs:label>Alpes de Murzsteg</rdfs:label>
    </owl:NamedIndividual>
    


    <!-- http://purl.obolibrary.org/obo/GAZ_00060637 -->

    <owl:NamedIndividual rdf:about="http://purl.obolibrary.org/obo/GAZ_00060637">
        <obo:RO_0001025 rdf:resource="http://purl.obolibrary.org/obo/GAZ_00051915"/>
        <obo:IAO_0000115>Un massif des Prealpes orientales septentrionales. Il s&apos;eleve en Autriche (limite entre la Basse-Autriche et le land de Styrie). Le massif est entoure par le Wienerwald et les Alpes de Gutenstein a l&apos;est, les Alpes de Murzsteg au sud et les Alpes d&apos;Ybbstal a l&apos;ouest.</obo:IAO_0000115>
        <oboInOwl:hasOBONamespace>GAZ</oboInOwl:hasOBONamespace>
        <oboInOwl:id>GAZ:00060637</oboInOwl:id>
        <rdfs:label>Alpes de Turnitz</rdfs:label>
    </owl:NamedIndividual>
    


    <!-- http://purl.obolibrary.org/obo/GAZ_00060638 -->

    <owl:NamedIndividual rdf:about="http://purl.obolibrary.org/obo/GAZ_00060638">
        <obo:RO_0001025 rdf:resource="http://purl.obolibrary.org/obo/GAZ_00051915"/>
        <obo:IAO_0000115>Un massif des Prealpes orientales septentrionales. Il s&apos;eleve en Autriche (limite entre le Land de Styrie, la Haute-Autriche et la Basse-Autriche). Le massif est entoure par les Alpes de Turnitz a l&apos;est, le massif du Hochschwab au sud, les Alpes d&apos;Ennstal au sud-ouest et les Peealpes de Haute-Autriche a l&apos;ouest. Il est borde par l&apos;Enns au sud-ouest. Il est egalement traverse par l&apos;Ybbs. Il est constitue des chainons de Krauterin, Gostling, Konigsberg, Eisenwurzen, Tormauer.</obo:IAO_0000115>
        <oboInOwl:hasOBONamespace>GAZ</oboInOwl:hasOBONamespace>
        <oboInOwl:id>GAZ:00060638</oboInOwl:id>
        <rdfs:label>Alpes d&apos;Ybbstal</rdfs:label>
    </owl:NamedIndividual>
    


    <!-- http://purl.obolibrary.org/obo/GAZ_00060639 -->

    <owl:NamedIndividual rdf:about="http://purl.obolibrary.org/obo/GAZ_00060639">
        <obo:RO_0001025 rdf:resource="http://purl.obolibrary.org/obo/GAZ_00051915"/>
        <obo:IAO_0000115>Un massif des Prealpes orientales septentrionales. Il s&apos;eleve en Autriche (Land de Styrie). Le massif est entoure par les Alpes d&apos;Ybbstal au nord, les Alpes de Murzsteg a l&apos;est, les Alpes de Lavanttal au sud et les Alpes d&apos;Ennstal a l&apos;ouest. Il est borde par la Mur au sud et l&apos;Enns au nord-ouest.</obo:IAO_0000115>
        <oboInOwl:hasOBONamespace>GAZ</oboInOwl:hasOBONamespace>
        <oboInOwl:id>GAZ:00060639</oboInOwl:id>
        <rdfs:label>Massif du Hochschwab</rdfs:label>
    </owl:NamedIndividual>
    


    <!-- http://purl.obolibrary.org/obo/GAZ_00060640 -->

    <owl:NamedIndividual rdf:about="http://purl.obolibrary.org/obo/GAZ_00060640">
        <obo:RO_0001025 rdf:resource="http://purl.obolibrary.org/obo/GAZ_00051915"/>
        <obo:IAO_0000115>Un massif des Prealpes orientales septentrionales. Il s&apos;eleve en Autriche (Haute-Autriche). Le massif est entoure par les Alpes d&apos;Ybbstal a l&apos;est, les Alpes d&apos;Ennstal et le massif mort au sud et le massif du Salzkammergut a l&apos;ouest. Il est traverse par l&apos;Enns et la Steyr en direction du nord.</obo:IAO_0000115>
        <oboInOwl:hasOBONamespace>GAZ</oboInOwl:hasOBONamespace>
        <oboInOwl:id>GAZ:00060640</oboInOwl:id>
        <rdfs:label>Prealpes de Haute-Autriche</rdfs:label>
    </owl:NamedIndividual>
    


    <!-- http://purl.obolibrary.org/obo/GAZ_00060641 -->

    <owl:NamedIndividual rdf:about="http://purl.obolibrary.org/obo/GAZ_00060641">
        <obo:RO_0001025 rdf:resource="http://purl.obolibrary.org/obo/GAZ_00051915"/>
        <obo:IAO_0000115>Une chaine de montagnes fortement karstiques des Prealpes orientales septentrionales. Elle se situe entierement en Autriche, s&apos;etendant sur des portions du land de Salzbourg, de la Haute-Autriche et la Styrie.</obo:IAO_0000115>
        <oboInOwl:hasOBONamespace>GAZ</oboInOwl:hasOBONamespace>
        <oboInOwl:id>GAZ:00060641</oboInOwl:id>
        <rdfs:label>Massif du Dachstein</rdfs:label>
    </owl:NamedIndividual>
    


    <!-- http://purl.obolibrary.org/obo/GAZ_00060642 -->

    <owl:NamedIndividual rdf:about="http://purl.obolibrary.org/obo/GAZ_00060642">
        <obo:RO_0001025 rdf:resource="http://purl.obolibrary.org/obo/GAZ_00051915"/>
        <obo:IAO_0000115>Un massif des Prealpes orientales septentrionales. Il s&apos;eleve en Autriche (limite entre le Land de Salzbourg et la Haute-Autriche), au nord et a l&apos;ouest de la region du Salzkammergut. Le massif est entoure par les prealpes de Haute-Autriche a l&apos;est, le massif mort au sud-est, le massif du Dachstein au sud, le massif de Tennen au sud-ouest et les Alpes de Berchtesgaden e l&apos;ouest. Il est borde e l&apos;ouest par la Salzach.</obo:IAO_0000115>
        <oboInOwl:hasOBONamespace>GAZ</oboInOwl:hasOBONamespace>
        <oboInOwl:id>GAZ:00060642</oboInOwl:id>
        <rdfs:label>Massif du Salzkammergut</rdfs:label>
    </owl:NamedIndividual>
    


    <!-- http://purl.obolibrary.org/obo/GAZ_00060643 -->

    <owl:NamedIndividual rdf:about="http://purl.obolibrary.org/obo/GAZ_00060643">
        <obo:RO_0001025 rdf:resource="http://purl.obolibrary.org/obo/GAZ_00060642"/>
        <obo:IAO_0000115>A lake in the Massif du Salzkammergut.</obo:IAO_0000115>
        <oboInOwl:hasOBONamespace>GAZ</oboInOwl:hasOBONamespace>
        <oboInOwl:id>GAZ:00060643</oboInOwl:id>
        <rdfs:label>Fuschisee</rdfs:label>
    </owl:NamedIndividual>
    


    <!-- http://purl.obolibrary.org/obo/GAZ_00060644 -->

    <owl:NamedIndividual rdf:about="http://purl.obolibrary.org/obo/GAZ_00060644">
        <obo:RO_0001025 rdf:resource="http://purl.obolibrary.org/obo/GAZ_00051915"/>
        <obo:IAO_0000115>Un massif des Prealpes orientales septentrionales. Il s&apos;eleve en Autriche (Land de Salzbourg). Ce massif en forme de plateau de 60 km2, dont 37 km2 au dessus de 2000 m, est entoure par le massif du Salzkammergut au nord, le massif du Dachstein a l&apos;est, le Niedere Tauern au sud et les Alpes de Berchtesgadena a l&apos;ouest. Il est borde a l&apos;ouest par la Salzach.</obo:IAO_0000115>
        <oboInOwl:hasOBONamespace>GAZ</oboInOwl:hasOBONamespace>
        <oboInOwl:id>GAZ:00060644</oboInOwl:id>
        <rdfs:label>Massif de Tennen</rdfs:label>
    </owl:NamedIndividual>
    


    <!-- http://purl.obolibrary.org/obo/GAZ_00060645 -->

    <owl:NamedIndividual rdf:about="http://purl.obolibrary.org/obo/GAZ_00060645">
        <obo:RO_0001025 rdf:resource="http://purl.obolibrary.org/obo/GAZ_00051915"/>
        <obo:IAO_0000115>Deux massifs des Prealpes orientales septentrionales. Ils s&apos;elevent en Autriche (Land du Tyrol et Land de Salzbourg). Les massifs sont orientes grossierement est-ouest et sont relies par le Romersattel. Celui de Lofer est le plus septentrional. Ils sont entoures par les Alpes de Chiemgau au nord, les Alpes de Berchtesgaden a l&apos;est, les Alpes de Kitzbuhel au sud et le massif de l&apos;Empereur a l&apos;ouest.</obo:IAO_0000115>
        <oboInOwl:hasOBONamespace>GAZ</oboInOwl:hasOBONamespace>
        <oboInOwl:id>GAZ:00060645</oboInOwl:id>
        <rdfs:label>Massifs de Lofer et Leogang</rdfs:label>
    </owl:NamedIndividual>
    


    <!-- http://purl.obolibrary.org/obo/GAZ_00060646 -->

    <owl:NamedIndividual rdf:about="http://purl.obolibrary.org/obo/GAZ_00060646">
        <obo:RO_0001025 rdf:resource="http://purl.obolibrary.org/obo/GAZ_00060645"/>
        <oboInOwl:hasOBONamespace>GAZ</oboInOwl:hasOBONamespace>
        <oboInOwl:id>GAZ:00060646</oboInOwl:id>
        <rdfs:label>Leoganger Steinberge</rdfs:label>
    </owl:NamedIndividual>
    


    <!-- http://purl.obolibrary.org/obo/GAZ_00060647 -->

    <owl:NamedIndividual rdf:about="http://purl.obolibrary.org/obo/GAZ_00060647">
        <obo:RO_0001025 rdf:resource="http://purl.obolibrary.org/obo/GAZ_00060645"/>
        <obo:IAO_0000115>Eine Gebirgsgruppe der NOrdlichen Kalkalpen in den Ostalpen.</obo:IAO_0000115>
        <oboInOwl:hasOBONamespace>GAZ</oboInOwl:hasOBONamespace>
        <oboInOwl:id>GAZ:00060647</oboInOwl:id>
        <rdfs:label>Loferer Steinberge</rdfs:label>
    </owl:NamedIndividual>
    


    <!-- http://purl.obolibrary.org/obo/GAZ_00060648 -->

    <owl:NamedIndividual rdf:about="http://purl.obolibrary.org/obo/GAZ_00060648">
        <obo:RO_0001025 rdf:resource="http://purl.obolibrary.org/obo/GAZ_00060647"/>
        <obo:IAO_0000115>A lake.</obo:IAO_0000115>
        <oboInOwl:hasOBONamespace>GAZ</oboInOwl:hasOBONamespace>
        <oboInOwl:id>GAZ:00060648</oboInOwl:id>
        <rdfs:label>Pillersee</rdfs:label>
    </owl:NamedIndividual>
    


    <!-- http://purl.obolibrary.org/obo/GAZ_00060649 -->

    <owl:NamedIndividual rdf:about="http://purl.obolibrary.org/obo/GAZ_00060649">
        <obo:RO_0001025 rdf:resource="http://purl.obolibrary.org/obo/GAZ_00051915"/>
        <obo:IAO_0000115>Un massif des Prealpes orientales septentrionales. Il s&apos;eelee entre l&apos;Allemagne (Baviere) et l&apos;Autriche (Land du Tyrol et Land de Salzbourg). Le massif est entoure par les Alpes de Berchtesgaden au sud-est, les massifs de Lofer et Leogang et le massif de l&apos;Empereur au sud et les Prealpes bavaroises a l&apos;ouest. Il est borde a l&apos;ouest par l&apos;Inn.</obo:IAO_0000115>
        <oboInOwl:hasOBONamespace>GAZ</oboInOwl:hasOBONamespace>
        <oboInOwl:id>GAZ:00060649</oboInOwl:id>
        <rdfs:label>Alpes de Chiemgau</rdfs:label>
    </owl:NamedIndividual>
    


    <!-- http://purl.obolibrary.org/obo/GAZ_00060650 -->

    <owl:NamedIndividual rdf:about="http://purl.obolibrary.org/obo/GAZ_00060650">
        <obo:RO_0001025 rdf:resource="http://purl.obolibrary.org/obo/GAZ_00051915"/>
        <obo:IAO_0000115>Un massif entoure par les Alpes de Chiemgau au nord, le Loferer Steinberge a l&apos;est, les Alpes de Kitzbuhel au sud et les Alpes de Brandenberg a l&apos;ouest. Il est borde a l&apos;ouest par Inn.</obo:IAO_0000115>
        <oboInOwl:hasOBONamespace>GAZ</oboInOwl:hasOBONamespace>
        <oboInOwl:id>GAZ:00060650</oboInOwl:id>
        <rdfs:label>Kaisergebirge</rdfs:label>
    </owl:NamedIndividual>
    


    <!-- http://purl.obolibrary.org/obo/GAZ_00060651 -->

    <owl:NamedIndividual rdf:about="http://purl.obolibrary.org/obo/GAZ_00060651">
        <obo:RO_0001025 rdf:resource="http://purl.obolibrary.org/obo/GAZ_00051915"/>
        <obo:IAO_0000115>Un massif des Prealpes orientales septentrionales. Il s&apos;eleve en Autriche (Land du Tyrol). Le massif est entoure par les Prealpes bavaroises au nord, le massif de l&apos;Empereur a l&apos;est, les Alpes de Kitzbuhel au sud-est et les Karwendel a l&apos;ouest. Il est borde au sud-est par l&apos;Inn et baigne par le lac d&apos;Achen a l&apos;ouest.</obo:IAO_0000115>
        <oboInOwl:hasOBONamespace>GAZ</oboInOwl:hasOBONamespace>
        <oboInOwl:id>GAZ:00060651</oboInOwl:id>
        <rdfs:label>Alpes de Brandenberg</rdfs:label>
    </owl:NamedIndividual>
    


    <!-- http://purl.obolibrary.org/obo/GAZ_00060652 -->

    <owl:NamedIndividual rdf:about="http://purl.obolibrary.org/obo/GAZ_00060652">
        <obo:RO_0001025 rdf:resource="http://purl.obolibrary.org/obo/GAZ_00051915"/>
        <obo:IAO_0000115>Un massif des Prealpes orientales septentrionales. Il s&apos;eleve entre l&apos;Autriche (Land du Tyrol) et principalement l&apos;Allemagne (Baviere). Le massif est entoure par les Alpes d&apos;Ammergau a l&apos;ouest, le Wetterstein au sud-ouest, les Karwendel au sud, les Alpes de Brandenberg au sud-est et les Alpes de Chiemgau a l&apos;est. Il est borde a l&apos;est par l&apos;Inn. Il est egalement coupe en deux en direction du nord par l&apos;Isar.</obo:IAO_0000115>
        <oboInOwl:hasOBONamespace>GAZ</oboInOwl:hasOBONamespace>
        <oboInOwl:id>GAZ:00060652</oboInOwl:id>
        <rdfs:label>Bavarian Prealps</rdfs:label>
    </owl:NamedIndividual>
    


    <!-- http://purl.obolibrary.org/obo/GAZ_00060653 -->

    <owl:NamedIndividual rdf:about="http://purl.obolibrary.org/obo/GAZ_00060653">
        <obo:RO_0001025 rdf:resource="http://purl.obolibrary.org/obo/GAZ_00060652"/>
        <obo:IAO_0000115>A lake in the Prealpes Bavaroises.</obo:IAO_0000115>
        <oboInOwl:hasOBONamespace>GAZ</oboInOwl:hasOBONamespace>
        <oboInOwl:id>GAZ:00060653</oboInOwl:id>
        <rdfs:label>Walchensee</rdfs:label>
    </owl:NamedIndividual>
    


    <!-- http://purl.obolibrary.org/obo/GAZ_00060655 -->

    <owl:NamedIndividual rdf:about="http://purl.obolibrary.org/obo/GAZ_00060655">
        <obo:RO_0001025 rdf:resource="http://purl.obolibrary.org/obo/GAZ_00060652"/>
        <obo:IAO_0000115>A lake in the Bavarian Prealps.</obo:IAO_0000115>
        <oboInOwl:hasOBONamespace>GAZ</oboInOwl:hasOBONamespace>
        <oboInOwl:id>GAZ:00060655</oboInOwl:id>
        <rdfs:label>Tegernsee [lake]</rdfs:label>
    </owl:NamedIndividual>
    


    <!-- http://purl.obolibrary.org/obo/GAZ_00060656 -->

    <owl:NamedIndividual rdf:about="http://purl.obolibrary.org/obo/GAZ_00060656">
        <obo:RO_0001025 rdf:resource="http://purl.obolibrary.org/obo/GAZ_00051915"/>
        <obo:IAO_0000115>Un massif des Prealpes orientales septentrionales. Il s&apos;eleve entre l&apos;Autriche (Land du Tyrol) et l&apos;Allemagne (Baviere). Le massif est entoure par les Prealpes bavaroises au nord-est, les Karwendel a l&apos;est, les Alpes de Stubai au sud, les Alpes de l&apos;Otztal au sud-ouest, les Alpes de Lechtal a l&apos;ouest et les Alpes d&apos;Ammergau au nord-ouest. Il est borde au sud par l&apos;Inn et a l&apos;ouest et au nord-ouest par le Loisach. Il est egalement traverse en direction de l&apos;est par le Leutascher Ache. Au sud de ce dernier, on distingue habituellement le chainon de Mieming (Mieminger Kette) du reste du massif.</obo:IAO_0000115>
        <oboInOwl:hasOBONamespace>GAZ</oboInOwl:hasOBONamespace>
        <oboInOwl:id>GAZ:00060656</oboInOwl:id>
        <rdfs:label>Wetterstein</rdfs:label>
    </owl:NamedIndividual>
    


    <!-- http://purl.obolibrary.org/obo/GAZ_00060657 -->

    <owl:NamedIndividual rdf:about="http://purl.obolibrary.org/obo/GAZ_00060657">
        <obo:RO_0001025 rdf:resource="http://purl.obolibrary.org/obo/GAZ_00051915"/>
        <obo:IAO_0000115>Un massif des Prealpes orientales septentrionales. Elles s&apos;elevent entre l&apos;Autriche (Land du Tyrol) et l&apos;Allemagne (Baviere). Le massif est entoure par les Prealpes bavaroises a l&apos;est, le Wetterstein au sud-est, les Alpes de Lechtal au sud-ouest et les Alpes d&apos;Allgau a l&apos;ouest. Il est borde a l&apos;ouest par Lech.</obo:IAO_0000115>
        <oboInOwl:hasOBONamespace>GAZ</oboInOwl:hasOBONamespace>
        <oboInOwl:id>GAZ:00060657</oboInOwl:id>
        <rdfs:label>Alpes d&apos;Ammergau</rdfs:label>
    </owl:NamedIndividual>
    


    <!-- http://purl.obolibrary.org/obo/GAZ_00060658 -->

    <owl:NamedIndividual rdf:about="http://purl.obolibrary.org/obo/GAZ_00060658">
        <obo:RO_0001025 rdf:resource="http://purl.obolibrary.org/obo/GAZ_00051915"/>
        <obo:IAO_0000115>Un massif des Prealpes orientales septentrionales. Il s&apos;eleve en Autriche (Vorarlberg). Il donne sa source au Lech. Le massif est entoure par les Alpes d&apos;Allgau au nord-est, les Alpes de Lechtal a l&apos;est, le massif de Verwall au sud, le Ratikon au sud-ouest et le massif du Bregenzerwald au nord-ouest. Il se situe au sud du col de Hochtannberg et a l&apos;ouest du col de Flexen.</obo:IAO_0000115>
        <oboInOwl:hasOBONamespace>GAZ</oboInOwl:hasOBONamespace>
        <oboInOwl:id>GAZ:00060658</oboInOwl:id>
        <rdfs:label>Massif de Lechquellen</rdfs:label>
    </owl:NamedIndividual>
    


    <!-- http://purl.obolibrary.org/obo/GAZ_00060659 -->

    <owl:NamedIndividual rdf:about="http://purl.obolibrary.org/obo/GAZ_00060659">
        <obo:RO_0001025 rdf:resource="http://purl.obolibrary.org/obo/GAZ_00051915"/>
        <obo:IAO_0000115>Un massif des Prealpes orientales septentrionales. Il s&apos;eleve en Autriche (Vorarlberg), au sud-ouest de la region du Bregenzerwald. Le massif est entoure par les Alpes d&apos;Allgau au nord-est, le massif de Lechquellen au sud-est, le Ratikon au sud-ouest et les Prealpes appenzelloises a l&apos;ouest Il est borde par la rive droite du Rhin a l&apos;ouest.</obo:IAO_0000115>
        <oboInOwl:hasOBONamespace>GAZ</oboInOwl:hasOBONamespace>
        <oboInOwl:id>GAZ:00060659</oboInOwl:id>
        <rdfs:label>Massif du Bregenzerwald</rdfs:label>
    </owl:NamedIndividual>
    


    <!-- http://purl.obolibrary.org/obo/GAZ_00060677 -->

    <owl:NamedIndividual rdf:about="http://purl.obolibrary.org/obo/GAZ_00060677">
        <obo:RO_0001025 rdf:resource="http://purl.obolibrary.org/obo/GAZ_00060705"/>
        <obo:IAO_0000115>Un lac de barrage situe sur la Dranse de Morzine dans la Vallee d&apos;Aulps, au dessus de Gorges du Pont-du-Diable.</obo:IAO_0000115>
        <oboInOwl:hasOBONamespace>GAZ</oboInOwl:hasOBONamespace>
        <oboInOwl:id>GAZ:00060677</oboInOwl:id>
        <rdfs:label>Lac du Jotty</rdfs:label>
    </owl:NamedIndividual>
    


    <!-- http://purl.obolibrary.org/obo/GAZ_00060678 -->

    <owl:NamedIndividual rdf:about="http://purl.obolibrary.org/obo/GAZ_00060678">
        <obo:RO_0001025 rdf:resource="http://purl.obolibrary.org/obo/GAZ_00060581"/>
        <obo:IAO_0000115>Un lac situe a 1384 m a l&apos;ouest des Cornettes de Bise.</obo:IAO_0000115>
        <oboInOwl:hasOBONamespace>GAZ</oboInOwl:hasOBONamespace>
        <oboInOwl:id>GAZ:00060678</oboInOwl:id>
        <rdfs:label>Lac de Fontaine</rdfs:label>
    </owl:NamedIndividual>
    


    <!-- http://purl.obolibrary.org/obo/GAZ_00060679 -->

    <owl:NamedIndividual rdf:about="http://purl.obolibrary.org/obo/GAZ_00060679">
        <obo:RO_0001025 rdf:resource="http://purl.obolibrary.org/obo/GAZ_00060581"/>
        <obo:IAO_0000115>A lake.</obo:IAO_0000115>
        <oboInOwl:hasOBONamespace>GAZ</oboInOwl:hasOBONamespace>
        <oboInOwl:id>GAZ:00060679</oboInOwl:id>
        <rdfs:label>Lac de Tavaneuse</rdfs:label>
    </owl:NamedIndividual>
    


    <!-- http://purl.obolibrary.org/obo/GAZ_00060680 -->

    <owl:NamedIndividual rdf:about="http://purl.obolibrary.org/obo/GAZ_00060680">
        <obo:RO_0001025 rdf:resource="http://purl.obolibrary.org/obo/GAZ_00060581"/>
        <obo:IAO_0000115>A lake.</obo:IAO_0000115>
        <oboInOwl:hasOBONamespace>GAZ</oboInOwl:hasOBONamespace>
        <oboInOwl:id>GAZ:00060680</oboInOwl:id>
        <rdfs:label>Lac de Montriond</rdfs:label>
    </owl:NamedIndividual>
    


    <!-- http://purl.obolibrary.org/obo/GAZ_00060681 -->

    <owl:NamedIndividual rdf:about="http://purl.obolibrary.org/obo/GAZ_00060681">
        <obo:RO_0001025 rdf:resource="http://purl.obolibrary.org/obo/GAZ_00060581"/>
        <obo:IAO_0000115>A lake.</obo:IAO_0000115>
        <oboInOwl:hasOBONamespace>GAZ</oboInOwl:hasOBONamespace>
        <oboInOwl:id>GAZ:00060681</oboInOwl:id>
        <rdfs:label>Lac des Plagnes</rdfs:label>
    </owl:NamedIndividual>
    


    <!-- http://purl.obolibrary.org/obo/GAZ_00060682 -->

    <owl:NamedIndividual rdf:about="http://purl.obolibrary.org/obo/GAZ_00060682">
        <obo:RO_0001025 rdf:resource="http://purl.obolibrary.org/obo/GAZ_00060581"/>
        <obo:IAO_0000115>A lake.</obo:IAO_0000115>
        <oboInOwl:hasOBONamespace>GAZ</oboInOwl:hasOBONamespace>
        <oboInOwl:id>GAZ:00060682</oboInOwl:id>
        <rdfs:label>Lac de Bise</rdfs:label>
    </owl:NamedIndividual>
    


    <!-- http://purl.obolibrary.org/obo/GAZ_00060683 -->

    <owl:NamedIndividual rdf:about="http://purl.obolibrary.org/obo/GAZ_00060683">
        <obo:RO_0001025 rdf:resource="http://purl.obolibrary.org/obo/GAZ_00060581"/>
        <obo:IAO_0000115>A lake. C&apos;est un lac artificiel, pour ne pas dire accidentel. En effet, en 1943, un enorme glissement de terrain provenant du lieu-dit &quot;Vallonet&quot;, emportant au passage de nombreuses maisons, a bloque l&apos;ecoulement du Brevon, donnant ainsi naissance au lac en meme temps qu&apos;il engloutissait des habitations.</obo:IAO_0000115>
        <oboInOwl:hasOBONamespace>GAZ</oboInOwl:hasOBONamespace>
        <oboInOwl:id>GAZ:00060683</oboInOwl:id>
        <rdfs:label>Lac de Vallon</rdfs:label>
    </owl:NamedIndividual>
    


    <!-- http://purl.obolibrary.org/obo/GAZ_00060684 -->

    <owl:NamedIndividual rdf:about="http://purl.obolibrary.org/obo/GAZ_00060684">
        <obo:RO_0001025 rdf:resource="http://purl.obolibrary.org/obo/GAZ_00060581"/>
        <obo:IAO_0000115>A lake.</obo:IAO_0000115>
        <oboInOwl:hasOBONamespace>GAZ</oboInOwl:hasOBONamespace>
        <oboInOwl:id>GAZ:00060684</oboInOwl:id>
        <rdfs:label>Lac de la Mouille</rdfs:label>
    </owl:NamedIndividual>
    


    <!-- http://purl.obolibrary.org/obo/GAZ_00060685 -->

    <owl:NamedIndividual rdf:about="http://purl.obolibrary.org/obo/GAZ_00060685">
        <obo:RO_0001025 rdf:resource="http://purl.obolibrary.org/obo/GAZ_00060581"/>
        <obo:IAO_0000115>A lake.</obo:IAO_0000115>
        <oboInOwl:hasOBONamespace>GAZ</oboInOwl:hasOBONamespace>
        <oboInOwl:id>GAZ:00060685</oboInOwl:id>
        <rdfs:label>Lac de Darbon</rdfs:label>
    </owl:NamedIndividual>
    


    <!-- http://purl.obolibrary.org/obo/GAZ_00060686 -->

    <owl:NamedIndividual rdf:about="http://purl.obolibrary.org/obo/GAZ_00060686">
        <obo:RO_0001025 rdf:resource="http://purl.obolibrary.org/obo/GAZ_00060581"/>
        <obo:IAO_0000115>A lake.</obo:IAO_0000115>
        <oboInOwl:hasOBONamespace>GAZ</oboInOwl:hasOBONamespace>
        <oboInOwl:id>GAZ:00060686</oboInOwl:id>
        <rdfs:label>Lac d&apos;Avoriaz</rdfs:label>
    </owl:NamedIndividual>
    


    <!-- http://purl.obolibrary.org/obo/GAZ_00060687 -->

    <owl:NamedIndividual rdf:about="http://purl.obolibrary.org/obo/GAZ_00060687">
        <obo:RO_0001025 rdf:resource="http://purl.obolibrary.org/obo/GAZ_00060691"/>
        <obo:IAO_0000115>A lake in the Haute-Savoie.</obo:IAO_0000115>
        <oboInOwl:hasOBONamespace>GAZ</oboInOwl:hasOBONamespace>
        <oboInOwl:id>GAZ:00060687</oboInOwl:id>
        <rdfs:label>Lac d&apos;Arvouin</rdfs:label>
    </owl:NamedIndividual>
    


    <!-- http://purl.obolibrary.org/obo/GAZ_00060688 -->

    <owl:NamedIndividual rdf:about="http://purl.obolibrary.org/obo/GAZ_00060688">
        <obo:RO_0001025 rdf:resource="http://purl.obolibrary.org/obo/GAZ_00060581"/>
        <obo:IAO_0000115>A lake. C&apos;est un petit lac artificiel cree en 1974 sur une zone naturelle humide a 1242 m.</obo:IAO_0000115>
        <oboInOwl:hasOBONamespace>GAZ</oboInOwl:hasOBONamespace>
        <oboInOwl:id>GAZ:00060688</oboInOwl:id>
        <rdfs:label>Lac de Vonnes</rdfs:label>
    </owl:NamedIndividual>
    


    <!-- http://purl.obolibrary.org/obo/GAZ_00060689 -->

    <owl:NamedIndividual rdf:about="http://purl.obolibrary.org/obo/GAZ_00060689">
        <obo:RO_0001025 rdf:resource="http://purl.obolibrary.org/obo/GAZ_00060581"/>
        <obo:IAO_0000115>A lake.</obo:IAO_0000115>
        <oboInOwl:hasOBONamespace>GAZ</oboInOwl:hasOBONamespace>
        <oboInOwl:id>GAZ:00060689</oboInOwl:id>
        <rdfs:label>Lac de la Case</rdfs:label>
    </owl:NamedIndividual>
    


    <!-- http://purl.obolibrary.org/obo/GAZ_00060690 -->

    <owl:NamedIndividual rdf:about="http://purl.obolibrary.org/obo/GAZ_00060690">
        <obo:RO_0001025 rdf:resource="http://purl.obolibrary.org/obo/GAZ_00060581"/>
        <obo:IAO_0000115>Une petite region du Chablais francais, constituee par le bassin versant de la Dranse d&apos;Abondance. Il s&apos;etend sur environ 25 km de Chevenoz jusqu&apos;a Chatel.</obo:IAO_0000115>
        <oboInOwl:hasOBONamespace>GAZ</oboInOwl:hasOBONamespace>
        <oboInOwl:id>GAZ:00060690</oboInOwl:id>
        <rdfs:label>Val d&apos;Abondance</rdfs:label>
    </owl:NamedIndividual>
    


    <!-- http://purl.obolibrary.org/obo/GAZ_00060691 -->

    <owl:NamedIndividual rdf:about="http://purl.obolibrary.org/obo/GAZ_00060691">
        <obo:RO_0001025 rdf:resource="http://purl.obolibrary.org/obo/GAZ_00060690"/>
        <obo:IAO_0000115>Petite riviere impetueuse de Haute-Savoie, elle prend sa source au-dessus du hameau de Plaine-Dranse (commune de Chatel) pres de la Pointe de Chesery et de la frontiere Franco-Suisse, dans le Chablais. Elle irrigue le Val d&apos;Abondance.</obo:IAO_0000115>
        <oboInOwl:hasOBONamespace>GAZ</oboInOwl:hasOBONamespace>
        <oboInOwl:id>GAZ:00060691</oboInOwl:id>
        <rdfs:label>Dranse d&apos;Abondance</rdfs:label>
    </owl:NamedIndividual>
    


    <!-- http://purl.obolibrary.org/obo/GAZ_00060704 -->

    <owl:NamedIndividual rdf:about="http://purl.obolibrary.org/obo/GAZ_00060704">
        <obo:RO_0001025 rdf:resource="http://purl.obolibrary.org/obo/GAZ_00060581"/>
        <obo:IAO_0000115>Une petite region du Chablais francais, constituee par le bassin versant de la Dranse de Morzine. Il s&apos;etend sur environ 25 km de La Vernaz jusqu&apos;a Morzine.</obo:IAO_0000115>
        <oboInOwl:hasOBONamespace>GAZ</oboInOwl:hasOBONamespace>
        <oboInOwl:id>GAZ:00060704</oboInOwl:id>
        <rdfs:label>Vallee d&apos;Aulps</rdfs:label>
    </owl:NamedIndividual>
    


    <!-- http://purl.obolibrary.org/obo/GAZ_00060705 -->

    <owl:NamedIndividual rdf:about="http://purl.obolibrary.org/obo/GAZ_00060705">
        <obo:RO_0001025 rdf:resource="http://purl.obolibrary.org/obo/GAZ_00060704"/>
        <obo:IAO_0000115>Une riviere francaise, petite mais impetueuse, qui coule dans le departement de la Haute-Savoie. Elle prend sa source sous le Col de Bossetant a la frontiere Franco-Suisse, dans le Chablais.</obo:IAO_0000115>
        <oboInOwl:hasOBONamespace>GAZ</oboInOwl:hasOBONamespace>
        <oboInOwl:id>GAZ:00060705</oboInOwl:id>
        <rdfs:label>Dranse de Morzine</rdfs:label>
    </owl:NamedIndividual>
    


    <!-- http://purl.obolibrary.org/obo/GAZ_00060714 -->

    <owl:NamedIndividual rdf:about="http://purl.obolibrary.org/obo/GAZ_00060714">
        <obo:RO_0001025 rdf:resource="http://purl.obolibrary.org/obo/GAZ_00393510"/>
        <obo:IAO_0000115>An lac d&apos;altitude du massif des aiguilles Rouges, situe sur la commune de Chamonix-Mont-Blanc.</obo:IAO_0000115>
        <oboInOwl:hasOBONamespace>GAZ</oboInOwl:hasOBONamespace>
        <oboInOwl:id>GAZ:00060714</oboInOwl:id>
        <rdfs:label>Lac Blanc</rdfs:label>
    </owl:NamedIndividual>
    


    <!-- http://purl.obolibrary.org/obo/GAZ_00060715 -->

    <owl:NamedIndividual rdf:about="http://purl.obolibrary.org/obo/GAZ_00060715">
        <obo:RO_0001025 rdf:resource="http://purl.obolibrary.org/obo/GAZ_00393510"/>
        <obo:IAO_0000115>Un lac a 2127 m sur la commune de Chamonix. Il se situe en contrebas du sommet du Brevent.</obo:IAO_0000115>
        <oboInOwl:hasOBONamespace>GAZ</oboInOwl:hasOBONamespace>
        <oboInOwl:id>GAZ:00060715</oboInOwl:id>
        <rdfs:label>Lac du Brevent</rdfs:label>
    </owl:NamedIndividual>
    


    <!-- http://purl.obolibrary.org/obo/GAZ_00060717 -->

    <owl:NamedIndividual rdf:about="http://purl.obolibrary.org/obo/GAZ_00060717">
        <obo:RO_0001025 rdf:resource="http://purl.obolibrary.org/obo/GAZ_00060577"/>
        <obo:IAO_0000115>A lake in the Aiguilles Rouges.</obo:IAO_0000115>
        <oboInOwl:hasOBONamespace>GAZ</oboInOwl:hasOBONamespace>
        <oboInOwl:id>GAZ:00060717</oboInOwl:id>
        <rdfs:label>Lac de Tardevent</rdfs:label>
    </owl:NamedIndividual>
    


    <!-- http://purl.obolibrary.org/obo/GAZ_00060719 -->

    <owl:NamedIndividual rdf:about="http://purl.obolibrary.org/obo/GAZ_00060719">
        <obo:RO_0001025 rdf:resource="http://purl.obolibrary.org/obo/GAZ_00393510"/>
        <obo:IAO_0000115>A lake.</obo:IAO_0000115>
        <oboInOwl:hasOBONamespace>GAZ</oboInOwl:hasOBONamespace>
        <oboInOwl:id>GAZ:00060719</oboInOwl:id>
        <rdfs:label>Lac Cornu</rdfs:label>
    </owl:NamedIndividual>
    


    <!-- http://purl.obolibrary.org/obo/GAZ_00060721 -->

    <owl:NamedIndividual rdf:about="http://purl.obolibrary.org/obo/GAZ_00060721">
        <obo:RO_0001025 rdf:resource="http://purl.obolibrary.org/obo/GAZ_00393510"/>
        <obo:IAO_0000115>A lake.</obo:IAO_0000115>
        <oboInOwl:hasOBONamespace>GAZ</oboInOwl:hasOBONamespace>
        <oboInOwl:id>GAZ:00060721</oboInOwl:id>
        <rdfs:label>Lac Noir des aiguilles Rouges</rdfs:label>
    </owl:NamedIndividual>
    


    <!-- http://purl.obolibrary.org/obo/GAZ_00060723 -->

    <owl:NamedIndividual rdf:about="http://purl.obolibrary.org/obo/GAZ_00060723">
        <obo:RO_0001025 rdf:resource="http://purl.obolibrary.org/obo/GAZ_00060583"/>
        <obo:IAO_0000115>A lake.</obo:IAO_0000115>
        <oboInOwl:hasOBONamespace>GAZ</oboInOwl:hasOBONamespace>
        <oboInOwl:id>GAZ:00060723</oboInOwl:id>
        <rdfs:label>Lac des Confins</rdfs:label>
    </owl:NamedIndividual>
    


    <!-- http://purl.obolibrary.org/obo/GAZ_00060754 -->

    <owl:NamedIndividual rdf:about="http://purl.obolibrary.org/obo/GAZ_00060754">
        <obo:RO_0001025 rdf:resource="http://purl.obolibrary.org/obo/GAZ_00060755"/>
        <obo:IAO_0000115>Un lac a 1945 m, dans le petit Massif de Pormenaz.</obo:IAO_0000115>
        <oboInOwl:hasOBONamespace>GAZ</oboInOwl:hasOBONamespace>
        <oboInOwl:id>GAZ:00060754</oboInOwl:id>
        <rdfs:label>Lac de Pormenaz</rdfs:label>
    </owl:NamedIndividual>
    


    <!-- http://purl.obolibrary.org/obo/GAZ_00060755 -->

    <owl:NamedIndividual rdf:about="http://purl.obolibrary.org/obo/GAZ_00060755">
        <obo:RO_0001025 rdf:resource="http://purl.obolibrary.org/obo/GAZ_00060577"/>
        <obo:IAO_0000115>Un petit chainon cristalin domine par la Pointe Noire de Pormeraz (2 07 m). Il est situe sur les communes de Servoz et de Passy, en Haute-Savoie. Il appartient a l&apos;ensemble geologique des Aiguilles Rouges dont il constitue l&apos;extremite sud, mais est separe de celui-ci par le torrent et les gorges de la Diosaz. Le versant sud du massif appartient a la reserve naturelle de Passy.</obo:IAO_0000115>
        <oboInOwl:hasOBONamespace>GAZ</oboInOwl:hasOBONamespace>
        <oboInOwl:id>GAZ:00060755</oboInOwl:id>
        <rdfs:label>Massif de Pormenaz</rdfs:label>
    </owl:NamedIndividual>
    


    <!-- http://purl.obolibrary.org/obo/GAZ_00061575 -->

    <owl:NamedIndividual rdf:about="http://purl.obolibrary.org/obo/GAZ_00061575">
        <obo:IAO_0000115>A pumped-storage power station; a reservoir.</obo:IAO_0000115>
        <oboInOwl:hasOBONamespace>GAZ</oboInOwl:hasOBONamespace>
        <oboInOwl:id>GAZ:00061575</oboInOwl:id>
        <rdfs:label>Pumpspeicherkraftwerk Langenprozelten</rdfs:label>
    </owl:NamedIndividual>
    


    <!-- http://purl.obolibrary.org/obo/GAZ_00061639 -->

    <owl:NamedIndividual rdf:about="http://purl.obolibrary.org/obo/GAZ_00061639">
        <obo:RO_0001025 rdf:resource="http://purl.obolibrary.org/obo/GAZ_00060652"/>
        <obo:IAO_0000115>A lake in the Allgau region.</obo:IAO_0000115>
        <oboInOwl:hasOBONamespace>GAZ</oboInOwl:hasOBONamespace>
        <oboInOwl:id>GAZ:00061639</oboInOwl:id>
        <rdfs:label>Weissensee</rdfs:label>
    </owl:NamedIndividual>
    


    <!-- http://purl.obolibrary.org/obo/GAZ_00061688 -->

    <owl:NamedIndividual rdf:about="http://purl.obolibrary.org/obo/GAZ_00061688">
        <obo:RO_0001025 rdf:resource="http://purl.obolibrary.org/obo/GAZ_00051913"/>
        <obo:IAO_0000115>A mountain range, the eastward extension of the Eastern Alps. It is part of the Alpokalja area of Hungary. It is located close to the city of Sopron (Western Hungary).</obo:IAO_0000115>
        <oboInOwl:hasOBONamespace>GAZ</oboInOwl:hasOBONamespace>
        <oboInOwl:id>GAZ:00061688</oboInOwl:id>
        <rdfs:label>Sopron Mountains</rdfs:label>
    </owl:NamedIndividual>
    


    <!-- http://purl.obolibrary.org/obo/GAZ_00062270 -->

    <owl:NamedIndividual rdf:about="http://purl.obolibrary.org/obo/GAZ_00062270">
        <obo:RO_0001025 rdf:resource="http://purl.obolibrary.org/obo/GAZ_00013805"/>
        <obo:IAO_0000115>A lake in Liechtenstein. It was created by a flood of the Rhine River with enormous erosion in 1927. The lake lies on 435 m in the village of Bendern-Gamprin.</obo:IAO_0000115>
        <oboInOwl:hasOBONamespace>GAZ</oboInOwl:hasOBONamespace>
        <oboInOwl:id>GAZ:00062270</oboInOwl:id>
        <rdfs:label>Gampriner Seele</rdfs:label>
    </owl:NamedIndividual>
    


    <!-- http://purl.obolibrary.org/obo/GAZ_00062483 -->

    <owl:NamedIndividual rdf:about="http://purl.obolibrary.org/obo/GAZ_00062483">
        <obo:RO_0001025 rdf:resource="http://purl.obolibrary.org/obo/GAZ_00056807"/>
        <obo:IAO_0000115>A lake located in the Bohinj municipality in the north-west of the country, and is inside Triglav National Park. It lies on the Sava Bohinjka river. Lake Bohinj is 4.2 km long and 1 km at its maximum width. It is a glacial lake dammed by a moraine.</obo:IAO_0000115>
        <oboInOwl:hasOBONamespace>GAZ</oboInOwl:hasOBONamespace>
        <oboInOwl:id>GAZ:00062483</oboInOwl:id>
        <rdfs:label>Lake Bohinj</rdfs:label>
    </owl:NamedIndividual>
    


    <!-- http://purl.obolibrary.org/obo/GAZ_00062486 -->

    <owl:NamedIndividual rdf:about="http://purl.obolibrary.org/obo/GAZ_00062486">
        <obo:RO_0001025 rdf:resource="http://purl.obolibrary.org/obo/GAZ_00056805"/>
        <obo:IAO_0000115>A rocky hanging valley in the Julian Alps in Slovenia, below the sheer sides of mountains Tiarica and Zelnarica to the southwest of Triglav. It is above the tree line and is geologically Alpine Karst.</obo:IAO_0000115>
        <oboInOwl:hasOBONamespace>GAZ</oboInOwl:hasOBONamespace>
        <oboInOwl:id>GAZ:00062486</oboInOwl:id>
        <rdfs:label>Triglav Lakes Valley</rdfs:label>
    </owl:NamedIndividual>
    


    <!-- http://purl.obolibrary.org/obo/GAZ_00062487 -->

    <owl:NamedIndividual rdf:about="http://purl.obolibrary.org/obo/GAZ_00062487">
        <obo:RO_0001025 rdf:resource="http://purl.obolibrary.org/obo/GAZ_00062486"/>
        <obo:IAO_0000115>A lake in the Triglav Lakes Valley.</obo:IAO_0000115>
        <oboInOwl:hasOBONamespace>GAZ</oboInOwl:hasOBONamespace>
        <oboInOwl:id>GAZ:00062487</oboInOwl:id>
        <rdfs:label>Crno jezero</rdfs:label>
    </owl:NamedIndividual>
    


    <!-- http://purl.obolibrary.org/obo/GAZ_00062488 -->

    <owl:NamedIndividual rdf:about="http://purl.obolibrary.org/obo/GAZ_00062488">
        <obo:RO_0001025 rdf:resource="http://purl.obolibrary.org/obo/GAZ_00062486"/>
        <obo:IAO_0000115>Two interconnected lakes in the Triglav Lakes Valley.</obo:IAO_0000115>
        <oboInOwl:hasOBONamespace>GAZ</oboInOwl:hasOBONamespace>
        <oboInOwl:id>GAZ:00062488</oboInOwl:id>
        <rdfs:label>Dvojno jezero</rdfs:label>
    </owl:NamedIndividual>
    


    <!-- http://purl.obolibrary.org/obo/GAZ_00062489 -->

    <owl:NamedIndividual rdf:about="http://purl.obolibrary.org/obo/GAZ_00062489">
        <obo:RO_0001025 rdf:resource="http://purl.obolibrary.org/obo/GAZ_00062486"/>
        <obo:IAO_0000115>A lake in the Triglav Lakes Valley.</obo:IAO_0000115>
        <oboInOwl:hasOBONamespace>GAZ</oboInOwl:hasOBONamespace>
        <oboInOwl:id>GAZ:00062489</oboInOwl:id>
        <rdfs:label>Veliko jezero</rdfs:label>
    </owl:NamedIndividual>
    


    <!-- http://purl.obolibrary.org/obo/GAZ_00062490 -->

    <owl:NamedIndividual rdf:about="http://purl.obolibrary.org/obo/GAZ_00062490">
        <obo:RO_0001025 rdf:resource="http://purl.obolibrary.org/obo/GAZ_00062486"/>
        <obo:IAO_0000115>A lake in the Triglav Lakes Valley.</obo:IAO_0000115>
        <oboInOwl:hasOBONamespace>GAZ</oboInOwl:hasOBONamespace>
        <oboInOwl:id>GAZ:00062490</oboInOwl:id>
        <rdfs:label>Jezero v Podstenju</rdfs:label>
    </owl:NamedIndividual>
    


    <!-- http://purl.obolibrary.org/obo/GAZ_00064111 -->

    <owl:NamedIndividual rdf:about="http://purl.obolibrary.org/obo/GAZ_00064111">
        <obo:IAO_0000115>A reservoir on the Saane river at Rossiniere, in the Pays d&apos;Enhaut of the canton of Vaud, Switzerland.</obo:IAO_0000115>
        <oboInOwl:hasOBONamespace>GAZ</oboInOwl:hasOBONamespace>
        <oboInOwl:id>GAZ:00064111</oboInOwl:id>
        <rdfs:label>Lac du Vernex</rdfs:label>
    </owl:NamedIndividual>
    


    <!-- http://purl.obolibrary.org/obo/GAZ_00064113 -->

    <owl:NamedIndividual rdf:about="http://purl.obolibrary.org/obo/GAZ_00064113">
        <obo:IAO_0000115>A reservoir on the Saane/Sarine river between Lessoc and Montbovon in the Canton of Fribourg, Switzerland.</obo:IAO_0000115>
        <oboInOwl:hasOBONamespace>GAZ</oboInOwl:hasOBONamespace>
        <oboInOwl:id>GAZ:00064113</oboInOwl:id>
        <rdfs:label>Lac de Lessoc</rdfs:label>
    </owl:NamedIndividual>
    


    <!-- http://purl.obolibrary.org/obo/GAZ_00064114 -->

    <owl:NamedIndividual rdf:about="http://purl.obolibrary.org/obo/GAZ_00064114">
        <obo:IAO_0000115>A reservoir formed by a dam on the Saane/Sarine river S of the city of Fribourg, Switzerland.</obo:IAO_0000115>
        <oboInOwl:hasOBONamespace>GAZ</oboInOwl:hasOBONamespace>
        <oboInOwl:id>GAZ:00064114</oboInOwl:id>
        <rdfs:label>Lac de Perolles</rdfs:label>
    </owl:NamedIndividual>
    


    <!-- http://purl.obolibrary.org/obo/GAZ_00064115 -->

    <owl:NamedIndividual rdf:about="http://purl.obolibrary.org/obo/GAZ_00064115">
        <obo:IAO_0000115>An artificial lake formed by a barrage of the Saane/Sarine river in the canton of Fribourg, Switzerland. The barrages at Schiffenen were completed in 1963.</obo:IAO_0000115>
        <oboInOwl:hasOBONamespace>GAZ</oboInOwl:hasOBONamespace>
        <oboInOwl:id>GAZ:00064115</oboInOwl:id>
        <rdfs:label>Schiffenensee</rdfs:label>
    </owl:NamedIndividual>
    


    <!-- http://purl.obolibrary.org/obo/GAZ_00064163 -->

    <owl:NamedIndividual rdf:about="http://purl.obolibrary.org/obo/GAZ_00064163">
        <obo:RO_0001025 rdf:resource="http://purl.obolibrary.org/obo/GAZ_00057287"/>
        <obo:IAO_0000115>A high mountain pass in the Bernina Range of the Alps, in the canton of Graubunden in Switzerland. It connects St. Moritz in the Engadin valley with Poschiavo, and Tirano in the Valtellina in Italy, but the pass itself is located in Switzerland.</obo:IAO_0000115>
        <oboInOwl:hasOBONamespace>GAZ</oboInOwl:hasOBONamespace>
        <oboInOwl:id>GAZ:00064163</oboInOwl:id>
        <rdfs:label>Bernina Pass</rdfs:label>
    </owl:NamedIndividual>
    


    <!-- http://purl.obolibrary.org/obo/GAZ_00064164 -->

    <owl:NamedIndividual rdf:about="http://purl.obolibrary.org/obo/GAZ_00064164">
        <obo:RO_0001025 rdf:resource="http://purl.obolibrary.org/obo/GAZ_00064163"/>
        <obo:IAO_0000115>A reservoir at the Bernina pass in the Grisons, Switzerland. Its surface area is 1.50 km2. The current reservoir was formed by the two dams Scala and Arlas on the site of two natural lakes (Lago Bianco and Lago della Scala).</obo:IAO_0000115>
        <oboInOwl:hasOBONamespace>GAZ</oboInOwl:hasOBONamespace>
        <oboInOwl:id>GAZ:00064164</oboInOwl:id>
        <rdfs:label>Lago Bianco</rdfs:label>
    </owl:NamedIndividual>
    


    <!-- http://purl.obolibrary.org/obo/GAZ_00064286 -->

    <owl:NamedIndividual rdf:about="http://purl.obolibrary.org/obo/GAZ_00064286">
        <obo:RO_0001025 rdf:resource="http://purl.obolibrary.org/obo/GAZ_00009676"/>
        <obo:IAO_0000115>A high mountain pass across the Bernese Alps connecting Leukerbad in the canton of Valais in Switzerland with Kandersteg in the canton of Bern. The pass lies between the Daubenhorn (2942 m) in the west and the Plattenhornern (2855 m.) in the east. The pass is the west end of the Aar Massif and the east end of the Wildstrubel Massif. Near the pass is the Daubensee, which has no outlet above ground.</obo:IAO_0000115>
        <oboInOwl:hasOBONamespace>GAZ</oboInOwl:hasOBONamespace>
        <oboInOwl:id>GAZ:00064286</oboInOwl:id>
        <rdfs:label>Gemmi Pass</rdfs:label>
    </owl:NamedIndividual>
    


    <!-- http://purl.obolibrary.org/obo/GAZ_00064287 -->

    <owl:NamedIndividual rdf:about="http://purl.obolibrary.org/obo/GAZ_00064287">
        <obo:RO_0001025 rdf:resource="http://purl.obolibrary.org/obo/GAZ_00064286"/>
        <obo:IAO_0000115>A lake at Gemmi Pass in Valais, Switzerland. It has no outlet above ground.</obo:IAO_0000115>
        <oboInOwl:hasOBONamespace>GAZ</oboInOwl:hasOBONamespace>
        <oboInOwl:id>GAZ:00064287</oboInOwl:id>
        <rdfs:label>Daubensee</rdfs:label>
    </owl:NamedIndividual>
    


    <!-- http://purl.obolibrary.org/obo/GAZ_00064301 -->

    <owl:NamedIndividual rdf:about="http://purl.obolibrary.org/obo/GAZ_00064301">
        <obo:RO_0001025 rdf:resource="http://purl.obolibrary.org/obo/GAZ_00064303"/>
        <obo:IAO_0000115>A lake in the Alpstein range of the canton of Appenzell Innerrhoden, Switzerland.</obo:IAO_0000115>
        <oboInOwl:hasOBONamespace>GAZ</oboInOwl:hasOBONamespace>
        <oboInOwl:id>GAZ:00064301</oboInOwl:id>
        <rdfs:label>Seealpsee</rdfs:label>
    </owl:NamedIndividual>
    


    <!-- http://purl.obolibrary.org/obo/GAZ_00064302 -->

    <owl:NamedIndividual rdf:about="http://purl.obolibrary.org/obo/GAZ_00064302">
        <obo:RO_0001025 rdf:resource="http://purl.obolibrary.org/obo/GAZ_00064303"/>
        <obo:IAO_0000115>A lake in the Alpstein range of the canton of Appenzell Innerrhoden, Switzerland.</obo:IAO_0000115>
        <oboInOwl:hasOBONamespace>GAZ</oboInOwl:hasOBONamespace>
        <oboInOwl:id>GAZ:00064302</oboInOwl:id>
        <rdfs:label>Samtisersee</rdfs:label>
    </owl:NamedIndividual>
    


    <!-- http://purl.obolibrary.org/obo/GAZ_00064303 -->

    <owl:NamedIndividual rdf:about="http://purl.obolibrary.org/obo/GAZ_00064303">
        <obo:RO_0001025 rdf:resource="http://purl.obolibrary.org/obo/GAZ_00060621"/>
        <obo:IAO_0000115>A subrange of the Appenzell Alps. Divided into N, S and Central groups.</obo:IAO_0000115>
        <oboInOwl:hasOBONamespace>GAZ</oboInOwl:hasOBONamespace>
        <oboInOwl:id>GAZ:00064303</oboInOwl:id>
        <rdfs:label>Alpstein Range</rdfs:label>
    </owl:NamedIndividual>
    


    <!-- http://purl.obolibrary.org/obo/GAZ_00064304 -->

    <owl:NamedIndividual rdf:about="http://purl.obolibrary.org/obo/GAZ_00064304">
        <obo:RO_0001025 rdf:resource="http://purl.obolibrary.org/obo/GAZ_00064303"/>
        <obo:IAO_0000115>A lake in the Alpstein range of the canton of Appenzell Innerrhoden, Switzerland. It is located in a narrow valley between Hundsteingrat and Roslen-Saxer First.</obo:IAO_0000115>
        <oboInOwl:hasOBONamespace>GAZ</oboInOwl:hasOBONamespace>
        <oboInOwl:id>GAZ:00064304</oboInOwl:id>
        <rdfs:label>Falensee</rdfs:label>
    </owl:NamedIndividual>
    


    <!-- http://purl.obolibrary.org/obo/GAZ_00064305 -->

    <owl:NamedIndividual rdf:about="http://purl.obolibrary.org/obo/GAZ_00064305">
        <obo:RO_0001025 rdf:resource="http://purl.obolibrary.org/obo/GAZ_00060621"/>
        <obo:IAO_0000115>A subrange of the Appenzell Alps.</obo:IAO_0000115>
        <oboInOwl:hasOBONamespace>GAZ</oboInOwl:hasOBONamespace>
        <oboInOwl:id>GAZ:00064305</oboInOwl:id>
        <rdfs:label>Churfirsten Range</rdfs:label>
    </owl:NamedIndividual>
    


    <!-- http://purl.obolibrary.org/obo/GAZ_00064306 -->

    <owl:NamedIndividual rdf:about="http://purl.obolibrary.org/obo/GAZ_00064306">
        <obo:RO_0001025 rdf:resource="http://purl.obolibrary.org/obo/GAZ_00060621"/>
        <obo:IAO_0000115>A subrange of the Appenzell Alps.</obo:IAO_0000115>
        <oboInOwl:hasOBONamespace>GAZ</oboInOwl:hasOBONamespace>
        <oboInOwl:id>GAZ:00064306</oboInOwl:id>
        <rdfs:label>Alviergruppe</rdfs:label>
    </owl:NamedIndividual>
    


    <!-- http://purl.obolibrary.org/obo/GAZ_00064307 -->

    <owl:NamedIndividual rdf:about="http://purl.obolibrary.org/obo/GAZ_00064307">
        <obo:RO_0001025 rdf:resource="http://purl.obolibrary.org/obo/GAZ_00060621"/>
        <obo:IAO_0000115>A subrange of the Appenzell Alps.</obo:IAO_0000115>
        <oboInOwl:hasOBONamespace>GAZ</oboInOwl:hasOBONamespace>
        <oboInOwl:id>GAZ:00064307</oboInOwl:id>
        <rdfs:label>Speer - Mattstock Range</rdfs:label>
    </owl:NamedIndividual>
    


    <!-- http://purl.obolibrary.org/obo/GAZ_00064496 -->

    <owl:NamedIndividual rdf:about="http://purl.obolibrary.org/obo/GAZ_00064496">
        <obo:RO_0001025 rdf:resource="http://purl.obolibrary.org/obo/GAZ_00057287"/>
        <obo:IAO_0000115>A lake below Piz Palu in the Grisons, Switzerland. Water from Palu Glacier feeds into the lake. In 1926, a dam was built enabling use of the lake as a reservoir.</obo:IAO_0000115>
        <oboInOwl:hasOBONamespace>GAZ</oboInOwl:hasOBONamespace>
        <oboInOwl:id>GAZ:00064496</oboInOwl:id>
        <rdfs:label>Lago Palu</rdfs:label>
    </owl:NamedIndividual>
    


    <!-- http://purl.obolibrary.org/obo/GAZ_00064505 -->

    <owl:NamedIndividual rdf:about="http://purl.obolibrary.org/obo/GAZ_00064505">
        <obo:RO_0001025 rdf:resource="http://purl.obolibrary.org/obo/GAZ_00057289"/>
        <obo:IAO_0000115>A group of tarn lakes in the Sesvenna Range near S-charl.</obo:IAO_0000115>
        <oboInOwl:hasOBONamespace>GAZ</oboInOwl:hasOBONamespace>
        <oboInOwl:id>GAZ:00064505</oboInOwl:id>
        <rdfs:label>Lais da Rims</rdfs:label>
    </owl:NamedIndividual>
    


    <!-- http://purl.obolibrary.org/obo/GAZ_00088601 -->

    <owl:NamedIndividual rdf:about="http://purl.obolibrary.org/obo/GAZ_00088601">
        <obo:RO_0001025 rdf:resource="http://purl.obolibrary.org/obo/GAZ_00056802"/>
        <obo:IAO_0000115>A national park in Styria, Austria. It is located west of the bend of the Enns River in Upper Styria, in the municipalities of Admont, Johnsbach, Weng, Hieflau, Landl, and Sankt Gallen, Styria.</obo:IAO_0000115>
        <oboInOwl:hasOBONamespace>GAZ</oboInOwl:hasOBONamespace>
        <oboInOwl:id>GAZ:00088601</oboInOwl:id>
        <rdfs:label>Gesause National Park</rdfs:label>
    </owl:NamedIndividual>
    


    <!-- http://purl.obolibrary.org/obo/GAZ_00088602 -->

    <owl:NamedIndividual rdf:about="http://purl.obolibrary.org/obo/GAZ_00088602">
        <obo:RO_0001025 rdf:resource="http://purl.obolibrary.org/obo/GAZ_00056784"/>
        <obo:IAO_0000115>A national park in the border area between the Federal Provinces of Carinthia, Salzburg and the Tyrol.</obo:IAO_0000115>
        <oboInOwl:hasOBONamespace>GAZ</oboInOwl:hasOBONamespace>
        <oboInOwl:id>GAZ:00088602</oboInOwl:id>
        <rdfs:label>Hohe Tauern National Park</rdfs:label>
    </owl:NamedIndividual>
    


    <!-- http://purl.obolibrary.org/obo/GAZ_00089859 -->

    <owl:NamedIndividual rdf:about="http://purl.obolibrary.org/obo/GAZ_00089859">
        <obo:RO_0001025 rdf:resource="http://purl.obolibrary.org/obo/GAZ_00009675"/>
        <obo:IAO_0000115>A massif delimited by the main valleys of rivers Drac, Romanche and Durance (with its Guisane dependency).</obo:IAO_0000115>
        <oboInOwl:hasOBONamespace>GAZ</oboInOwl:hasOBONamespace>
        <oboInOwl:id>GAZ:00089859</oboInOwl:id>
        <rdfs:label>Massif des Ecrins</rdfs:label>
    </owl:NamedIndividual>
    


    <!-- http://purl.obolibrary.org/obo/GAZ_00089884 -->

    <owl:NamedIndividual rdf:about="http://purl.obolibrary.org/obo/GAZ_00089884">
        <obo:RO_0001025 rdf:resource="http://purl.obolibrary.org/obo/GAZ_00056806"/>
        <oboInOwl:hasOBONamespace>GAZ</oboInOwl:hasOBONamespace>
        <oboInOwl:id>GAZ:00089884</oboInOwl:id>
        <rdfs:label>Parco Nazionale Dolomiti Bellunesi</rdfs:label>
    </owl:NamedIndividual>
    


    <!-- http://purl.obolibrary.org/obo/GAZ_00090209 -->

    <owl:NamedIndividual rdf:about="http://purl.obolibrary.org/obo/GAZ_00090209">
        <obo:RO_0001025 rdf:resource="http://purl.obolibrary.org/obo/GAZ_00090210"/>
        <obo:IAO_0000115>A national park that covers the Oosterscheld. Its boundaries are the dikes of Schouwen-Duiveland, Tholen and Sint-Philipsland, Noord-Beveland and Zuid-Beveland, and the dams of the Delta Works.</obo:IAO_0000115>
        <oboInOwl:hasOBONamespace>GAZ</oboInOwl:hasOBONamespace>
        <oboInOwl:id>GAZ:00090209</oboInOwl:id>
        <rdfs:label>Nationaal Park Oosterschelde</rdfs:label>
    </owl:NamedIndividual>
    


    <!-- http://purl.obolibrary.org/obo/GAZ_00090210 -->

    <owl:NamedIndividual rdf:about="http://purl.obolibrary.org/obo/GAZ_00090210">
        <obo:RO_0001025 rdf:resource="http://purl.obolibrary.org/obo/GAZ_00179752"/>
        <obo:IAO_0000115>A former estuary in Zeeland, the Netherlands, between Schouwen-Duiveland and Tholen on the north and Noord-Beveland and Zuid-Beveland on the south. Disconnected from the river by 1903.</obo:IAO_0000115>
        <oboInOwl:hasOBONamespace>GAZ</oboInOwl:hasOBONamespace>
        <oboInOwl:id>GAZ:00090210</oboInOwl:id>
        <rdfs:label>Oosterschelde</rdfs:label>
    </owl:NamedIndividual>
    


    <!-- http://purl.obolibrary.org/obo/GAZ_00090211 -->

    <owl:NamedIndividual rdf:about="http://purl.obolibrary.org/obo/GAZ_00090211">
        <obo:RO_0001025 rdf:resource="http://purl.obolibrary.org/obo/GAZ_00144376"/>
        <obo:IAO_0000115>One of the largest national parks of the Netherlands and one of the last freshwater tide areas in Europe.</obo:IAO_0000115>
        <oboInOwl:hasOBONamespace>GAZ</oboInOwl:hasOBONamespace>
        <oboInOwl:id>GAZ:00090211</oboInOwl:id>
        <rdfs:label>Nationaal Park De Biesbosch</rdfs:label>
    </owl:NamedIndividual>
    


    <!-- http://purl.obolibrary.org/obo/GAZ_00100717 -->

    <owl:NamedIndividual rdf:about="http://purl.obolibrary.org/obo/GAZ_00100717">
        <obo:RO_0001025 rdf:resource="http://purl.obolibrary.org/obo/GAZ_00056803"/>
        <obo:IAO_0000115>An artificial lake. Der Achensee liegt nordlich von Jenbach in Tirol. Er bildet mit dem Achental die Grenze zwischen Karwendelgebirge im Westen und Brandenberger Alpen im Osten.</obo:IAO_0000115>
        <oboInOwl:hasOBONamespace>GAZ</oboInOwl:hasOBONamespace>
        <oboInOwl:id>GAZ:00100717</oboInOwl:id>
        <rdfs:label>Achensee</rdfs:label>
    </owl:NamedIndividual>
    


    <!-- http://purl.obolibrary.org/obo/GAZ_00100720 -->

    <owl:NamedIndividual rdf:about="http://purl.obolibrary.org/obo/GAZ_00100720">
        <obo:RO_0001025 rdf:resource="http://purl.obolibrary.org/obo/GAZ_00056798"/>
        <obo:IAO_0000115>Ein Alpensee im steirischen Teil des Salzkammergutes in der NAhe von Bad Aussee.</obo:IAO_0000115>
        <oboInOwl:hasOBONamespace>GAZ</oboInOwl:hasOBONamespace>
        <oboInOwl:id>GAZ:00100720</oboInOwl:id>
        <rdfs:label>Grundlsee</rdfs:label>
    </owl:NamedIndividual>
    


    <!-- http://purl.obolibrary.org/obo/GAZ_00100730 -->

    <owl:NamedIndividual rdf:about="http://purl.obolibrary.org/obo/GAZ_00100730">
        <obo:RO_0001025 rdf:resource="http://purl.obolibrary.org/obo/GAZ_00056798"/>
        <obo:IAO_0000115>Ein Bergsee am Fusse des Toten Gebirges (Salzkammergut, Oberosterreich).</obo:IAO_0000115>
        <oboInOwl:hasOBONamespace>GAZ</oboInOwl:hasOBONamespace>
        <oboInOwl:id>GAZ:00100730</oboInOwl:id>
        <rdfs:label>Offensee</rdfs:label>
    </owl:NamedIndividual>
    


    <!-- http://purl.obolibrary.org/obo/GAZ_00100736 -->

    <owl:NamedIndividual rdf:about="http://purl.obolibrary.org/obo/GAZ_00100736">
        <obo:RO_0001025 rdf:resource="http://purl.obolibrary.org/obo/GAZ_00100737"/>
        <oboInOwl:hasOBONamespace>GAZ</oboInOwl:hasOBONamespace>
        <oboInOwl:id>GAZ:00100736</oboInOwl:id>
        <rdfs:label>Grosse Odsee</rdfs:label>
    </owl:NamedIndividual>
    


    <!-- http://purl.obolibrary.org/obo/GAZ_00100737 -->

    <owl:NamedIndividual rdf:about="http://purl.obolibrary.org/obo/GAZ_00100737">
        <obo:RO_0001025 rdf:resource="http://purl.obolibrary.org/obo/GAZ_00056798"/>
        <obo:IAO_0000115>Zwei zum Salzkammergut zahlende, im Gemeindegebiet von Grunau im Almtal, Oberosterreich gelegene, waldgesaumte Bergseen ohne oberirdische Zu- oder Abflusse.</obo:IAO_0000115>
        <oboInOwl:hasOBONamespace>GAZ</oboInOwl:hasOBONamespace>
        <oboInOwl:id>GAZ:00100737</oboInOwl:id>
        <rdfs:label>Odseen</rdfs:label>
    </owl:NamedIndividual>
    


    <!-- http://purl.obolibrary.org/obo/GAZ_00100738 -->

    <owl:NamedIndividual rdf:about="http://purl.obolibrary.org/obo/GAZ_00100738">
        <obo:RO_0001025 rdf:resource="http://purl.obolibrary.org/obo/GAZ_00100737"/>
        <oboInOwl:hasOBONamespace>GAZ</oboInOwl:hasOBONamespace>
        <oboInOwl:id>GAZ:00100738</oboInOwl:id>
        <rdfs:label>Kleine Odsee</rdfs:label>
    </owl:NamedIndividual>
    


    <!-- http://purl.obolibrary.org/obo/GAZ_00101704 -->

    <owl:NamedIndividual rdf:about="http://purl.obolibrary.org/obo/GAZ_00101704">
        <obo:RO_0001025 rdf:resource="http://purl.obolibrary.org/obo/GAZ_00056798"/>
        <obo:IAO_0000115>A lake. Liegt im Toten Gebirge auf der steirischen Seite des Salzkammergutes in Osterreich.</obo:IAO_0000115>
        <oboInOwl:hasOBONamespace>GAZ</oboInOwl:hasOBONamespace>
        <oboInOwl:id>GAZ:00101704</oboInOwl:id>
        <rdfs:label>Elmsee</rdfs:label>
    </owl:NamedIndividual>
    


    <!-- http://purl.obolibrary.org/obo/GAZ_00101705 -->

    <owl:NamedIndividual rdf:about="http://purl.obolibrary.org/obo/GAZ_00101705">
        <obo:RO_0001025 rdf:resource="http://purl.obolibrary.org/obo/GAZ_00056798"/>
        <obo:IAO_0000115>A lake. Im steirischen Teil des Salzkammergut im Toten Gebirge in der Nahe des Grundlsees.</obo:IAO_0000115>
        <oboInOwl:hasOBONamespace>GAZ</oboInOwl:hasOBONamespace>
        <oboInOwl:id>GAZ:00101705</oboInOwl:id>
        <rdfs:label>Lahngangseen</rdfs:label>
    </owl:NamedIndividual>
    


    <!-- http://purl.obolibrary.org/obo/GAZ_00101706 -->

    <owl:NamedIndividual rdf:about="http://purl.obolibrary.org/obo/GAZ_00101706">
        <obo:RO_0001025 rdf:resource="http://purl.obolibrary.org/obo/GAZ_00101705"/>
        <oboInOwl:hasOBONamespace>GAZ</oboInOwl:hasOBONamespace>
        <oboInOwl:id>GAZ:00101706</oboInOwl:id>
        <rdfs:label>Hinterer Lahngangsee</rdfs:label>
    </owl:NamedIndividual>
    


    <!-- http://purl.obolibrary.org/obo/GAZ_00101707 -->

    <owl:NamedIndividual rdf:about="http://purl.obolibrary.org/obo/GAZ_00101707">
        <obo:RO_0001025 rdf:resource="http://purl.obolibrary.org/obo/GAZ_00101705"/>
        <oboInOwl:hasOBONamespace>GAZ</oboInOwl:hasOBONamespace>
        <oboInOwl:id>GAZ:00101707</oboInOwl:id>
        <rdfs:label>Vorderer Lahngangsee</rdfs:label>
    </owl:NamedIndividual>
    


    <!-- http://purl.obolibrary.org/obo/GAZ_00101708 -->

    <owl:NamedIndividual rdf:about="http://purl.obolibrary.org/obo/GAZ_00101708">
        <obo:RO_0001025 rdf:resource="http://purl.obolibrary.org/obo/GAZ_00056798"/>
        <obo:IAO_0000115>A dimictic lake. Ein Alpensee im steirischen Salzkammergut (Osterreich) in der Nahe von Bad Aussee.</obo:IAO_0000115>
        <oboInOwl:hasOBONamespace>GAZ</oboInOwl:hasOBONamespace>
        <oboInOwl:id>GAZ:00101708</oboInOwl:id>
        <rdfs:label>Altausseer See</rdfs:label>
    </owl:NamedIndividual>
    


    <!-- http://purl.obolibrary.org/obo/GAZ_00101709 -->

    <owl:NamedIndividual rdf:about="http://purl.obolibrary.org/obo/GAZ_00101709">
        <obo:RO_0001025 rdf:resource="http://purl.obolibrary.org/obo/GAZ_00056798"/>
        <obo:IAO_0000115>Part of the Totes Gebirge mountain range in the Salzkammergut of Austria. It is a Nature Reserve, notable for its caves and unspoilt alpine Karst ecosystem. The central plateau area is relatively flat, at an altitude of 1500-1600 m, rising gently to the north and east, and covering about 4 km2. The whole massif is approximately 12 km2. The area drops steeply on all sides, and is bounded to the SE by path 234 from the Wildenseehutte down to Altausseer See, to the south by the lake itself, then to the SW by the road to Blaa-Alm. The Western edge is marked by the valley of Grune Bichl, and the northern limit is the ridge crest of Schonberg, then a rather ill-defined line back to the Wildenseehutte.</obo:IAO_0000115>
        <oboInOwl:hasOBONamespace>GAZ</oboInOwl:hasOBONamespace>
        <oboInOwl:id>GAZ:00101709</oboInOwl:id>
        <rdfs:label>Loser Plateau</rdfs:label>
    </owl:NamedIndividual>
    


    <!-- http://purl.obolibrary.org/obo/GAZ_00102567 -->

    <owl:NamedIndividual rdf:about="http://purl.obolibrary.org/obo/GAZ_00102567">
        <obo:RO_0001025 rdf:resource="http://purl.obolibrary.org/obo/GAZ_00056786"/>
        <obo:IAO_0000115>Eine Untergruppe der Zentralalpen in den Ostalpen. Zusammen mit den Radstadter Tauern, den Rottenmanner und Wolzer Tauern und den Seckauer Tauern bilden die Schladminger Tauern die Grossgruppe der Niederen Tauern. Das Gebirge befindet sich in Osterreich in den Bundeslandern Salzburg und Steiermark.</obo:IAO_0000115>
        <oboInOwl:hasOBONamespace>GAZ</oboInOwl:hasOBONamespace>
        <oboInOwl:id>GAZ:00102567</oboInOwl:id>
        <rdfs:label>Schladminger Tauern</rdfs:label>
    </owl:NamedIndividual>
    


    <!-- http://purl.obolibrary.org/obo/GAZ_00102568 -->

    <owl:NamedIndividual rdf:about="http://purl.obolibrary.org/obo/GAZ_00102568">
        <obo:RO_0001025 rdf:resource="http://purl.obolibrary.org/obo/GAZ_00051914"/>
        <obo:IAO_0000115>A part of the Central Eastern Alps.</obo:IAO_0000115>
        <oboInOwl:hasOBONamespace>GAZ</oboInOwl:hasOBONamespace>
        <oboInOwl:id>GAZ:00102568</oboInOwl:id>
        <rdfs:label>Randgebirge ostlich der Mur</rdfs:label>
    </owl:NamedIndividual>
    


    <!-- http://purl.obolibrary.org/obo/GAZ_00103422 -->

    <owl:NamedIndividual rdf:about="http://purl.obolibrary.org/obo/GAZ_00103422">
        <obo:RO_0001025 rdf:resource="http://purl.obolibrary.org/obo/GAZ_00056790"/>
        <obo:IAO_0000115>Ein Bergsee in den Stubaier Alpen. Er liegt nordostlich vom Wilden Pfaff in 2.289 m Hohe unweit der Sulzenauhutte. Er ist durch das Abschmelzen des Sulzenauferners entstanden und wird von einem Seitenarm des Sulzenaubaches entwassert.</obo:IAO_0000115>
        <oboInOwl:hasOBONamespace>GAZ</oboInOwl:hasOBONamespace>
        <oboInOwl:id>GAZ:00103422</oboInOwl:id>
        <rdfs:label>Blaue Lacke</rdfs:label>
    </owl:NamedIndividual>
    


    <!-- http://purl.obolibrary.org/obo/GAZ_00103424 -->

    <owl:NamedIndividual rdf:about="http://purl.obolibrary.org/obo/GAZ_00103424">
        <obo:RO_0001025 rdf:resource="http://purl.obolibrary.org/obo/GAZ_00056790"/>
        <obo:IAO_0000115>Ein Bergsee in den Stubaier Alpen.</obo:IAO_0000115>
        <oboInOwl:hasOBONamespace>GAZ</oboInOwl:hasOBONamespace>
        <oboInOwl:id>GAZ:00103424</oboInOwl:id>
        <rdfs:label>Grunausee</rdfs:label>
    </owl:NamedIndividual>
    


    <!-- http://purl.obolibrary.org/obo/GAZ_00103425 -->

    <owl:NamedIndividual rdf:about="http://purl.obolibrary.org/obo/GAZ_00103425">
        <obo:RO_0001025 rdf:resource="http://purl.obolibrary.org/obo/GAZ_00056787"/>
        <obo:IAO_0000115>Der grosste See in den Otztaler Alpen.</obo:IAO_0000115>
        <oboInOwl:hasOBONamespace>GAZ</oboInOwl:hasOBONamespace>
        <oboInOwl:id>GAZ:00103425</oboInOwl:id>
        <rdfs:label>Rifflsee</rdfs:label>
    </owl:NamedIndividual>
    


    <!-- http://purl.obolibrary.org/obo/GAZ_00103426 -->

    <owl:NamedIndividual rdf:about="http://purl.obolibrary.org/obo/GAZ_00103426">
        <obo:RO_0001025 rdf:resource="http://purl.obolibrary.org/obo/GAZ_00056787"/>
        <obo:IAO_0000115>Ein Bergsee im Geigenkamm in den Otztaler Alpen. Es handelt sich hierbei um einen Karsee, er liegt auf einer Hohe von 2525 m oberhalb des Pitztals und nordwestlich des Hundstalkogels.</obo:IAO_0000115>
        <oboInOwl:hasOBONamespace>GAZ</oboInOwl:hasOBONamespace>
        <oboInOwl:id>GAZ:00103426</oboInOwl:id>
        <rdfs:label>Moalandlsee</rdfs:label>
    </owl:NamedIndividual>
    


    <!-- http://purl.obolibrary.org/obo/GAZ_00103428 -->

    <owl:NamedIndividual rdf:about="http://purl.obolibrary.org/obo/GAZ_00103428">
        <obo:RO_0001025 rdf:resource="http://purl.obolibrary.org/obo/GAZ_00056785"/>
        <obo:IAO_0000115>Ein kleiner Moorsee in den Kitzbuheler Alpen. Er gilt als warmster Moorsee Tirols.</obo:IAO_0000115>
        <oboInOwl:hasOBONamespace>GAZ</oboInOwl:hasOBONamespace>
        <oboInOwl:id>GAZ:00103428</oboInOwl:id>
        <rdfs:label>Schwarzsee</rdfs:label>
    </owl:NamedIndividual>
    


    <!-- http://purl.obolibrary.org/obo/GAZ_00103429 -->

    <owl:NamedIndividual rdf:about="http://purl.obolibrary.org/obo/GAZ_00103429">
        <obo:RO_0001025 rdf:resource="http://purl.obolibrary.org/obo/GAZ_00056800"/>
        <obo:IAO_0000115>Ein 1.631 m u. A. hoch gelegener kleiner Stausee oberhalb des Vilsalpsee in den Allgauer Alpen bei Tannheim in Tirol.</obo:IAO_0000115>
        <oboInOwl:hasOBONamespace>GAZ</oboInOwl:hasOBONamespace>
        <oboInOwl:id>GAZ:00103429</oboInOwl:id>
        <rdfs:label>Traualpsee</rdfs:label>
    </owl:NamedIndividual>
    


    <!-- http://purl.obolibrary.org/obo/GAZ_00103433 -->

    <owl:NamedIndividual rdf:about="http://purl.obolibrary.org/obo/GAZ_00103433">
        <obo:RO_0001025 rdf:resource="http://purl.obolibrary.org/obo/GAZ_00057284"/>
        <obo:IAO_0000115>An artificial lake.</obo:IAO_0000115>
        <oboInOwl:hasOBONamespace>GAZ</oboInOwl:hasOBONamespace>
        <oboInOwl:id>GAZ:00103433</oboInOwl:id>
        <rdfs:label>Silvretta Lake</rdfs:label>
    </owl:NamedIndividual>
    


    <!-- http://purl.obolibrary.org/obo/GAZ_00103500 -->

    <owl:NamedIndividual rdf:about="http://purl.obolibrary.org/obo/GAZ_00103500">
        <obo:RO_0001025 rdf:resource="http://purl.obolibrary.org/obo/GAZ_00056784"/>
        <obo:RO_0001025 rdf:resource="http://purl.obolibrary.org/obo/GAZ_00088602"/>
        <obo:IAO_0000115>A reservoir.</obo:IAO_0000115>
        <oboInOwl:hasOBONamespace>GAZ</oboInOwl:hasOBONamespace>
        <oboInOwl:id>GAZ:00103500</oboInOwl:id>
        <rdfs:label>Stausee Margaritze</rdfs:label>
    </owl:NamedIndividual>
    


    <!-- http://purl.obolibrary.org/obo/GAZ_00103514 -->

    <owl:NamedIndividual rdf:about="http://purl.obolibrary.org/obo/GAZ_00103514">
        <obo:RO_0001025 rdf:resource="http://purl.obolibrary.org/obo/GAZ_00056784"/>
        <obo:IAO_0000115>A reservoir.</obo:IAO_0000115>
        <oboInOwl:hasOBONamespace>GAZ</oboInOwl:hasOBONamespace>
        <oboInOwl:id>GAZ:00103514</oboInOwl:id>
        <rdfs:label>Stausee Mooserboden</rdfs:label>
    </owl:NamedIndividual>
    


    <!-- http://purl.obolibrary.org/obo/GAZ_00103515 -->

    <owl:NamedIndividual rdf:about="http://purl.obolibrary.org/obo/GAZ_00103515">
        <obo:RO_0001025 rdf:resource="http://purl.obolibrary.org/obo/GAZ_00056784"/>
        <obo:IAO_0000115>A reservoir.</obo:IAO_0000115>
        <oboInOwl:hasOBONamespace>GAZ</oboInOwl:hasOBONamespace>
        <oboInOwl:id>GAZ:00103515</oboInOwl:id>
        <rdfs:label>Stausee Wasserfallboden</rdfs:label>
    </owl:NamedIndividual>
    


    <!-- http://purl.obolibrary.org/obo/GAZ_00103517 -->

    <owl:NamedIndividual rdf:about="http://purl.obolibrary.org/obo/GAZ_00103517">
        <obo:RO_0001025 rdf:resource="http://purl.obolibrary.org/obo/GAZ_00056784"/>
        <obo:IAO_0000115>Zwei Alpenseen im Osten der Hohen Tauern, die durch ihre besondere Lage und Farbung unter Bergsteigern und Wanderern bekannt sind.</obo:IAO_0000115>
        <oboInOwl:hasOBONamespace>GAZ</oboInOwl:hasOBONamespace>
        <oboInOwl:id>GAZ:00103517</oboInOwl:id>
        <rdfs:label>Rotguldenseen</rdfs:label>
    </owl:NamedIndividual>
    


    <!-- http://purl.obolibrary.org/obo/GAZ_00103533 -->

    <owl:NamedIndividual rdf:about="http://purl.obolibrary.org/obo/GAZ_00103533">
        <obo:RO_0001025 rdf:resource="http://purl.obolibrary.org/obo/GAZ_00060658"/>
        <obo:IAO_0000115>A reservoir.</obo:IAO_0000115>
        <oboInOwl:hasOBONamespace>GAZ</oboInOwl:hasOBONamespace>
        <oboInOwl:id>GAZ:00103533</oboInOwl:id>
        <rdfs:label>Spullersee</rdfs:label>
    </owl:NamedIndividual>
    


    <!-- http://purl.obolibrary.org/obo/GAZ_00103545 -->

    <owl:NamedIndividual rdf:about="http://purl.obolibrary.org/obo/GAZ_00103545">
        <obo:RO_0001025 rdf:resource="http://purl.obolibrary.org/obo/GAZ_00060626"/>
        <obo:IAO_0000115>Ein See in den Gurktaler Alpen in Karnten.</obo:IAO_0000115>
        <oboInOwl:hasOBONamespace>GAZ</oboInOwl:hasOBONamespace>
        <oboInOwl:id>GAZ:00103545</oboInOwl:id>
        <rdfs:label>Falkertsee</rdfs:label>
    </owl:NamedIndividual>
    


    <!-- http://purl.obolibrary.org/obo/GAZ_00103552 -->

    <owl:NamedIndividual rdf:about="http://purl.obolibrary.org/obo/GAZ_00103552">
        <obo:RO_0001025 rdf:resource="http://purl.obolibrary.org/obo/GAZ_00060626"/>
        <obo:IAO_0000115>Ein See liegt im Bereich der Gurktaler Alpen, nordlich von Feldkirchen in Karnten, in einem sehr windgeschutzen Becken.</obo:IAO_0000115>
        <oboInOwl:hasOBONamespace>GAZ</oboInOwl:hasOBONamespace>
        <oboInOwl:id>GAZ:00103552</oboInOwl:id>
        <rdfs:label>Goggausee</rdfs:label>
    </owl:NamedIndividual>
    


    <!-- http://purl.obolibrary.org/obo/GAZ_00103572 -->

    <owl:NamedIndividual rdf:about="http://purl.obolibrary.org/obo/GAZ_00103572">
        <obo:RO_0001025 rdf:resource="http://purl.obolibrary.org/obo/GAZ_00103573"/>
        <obo:IAO_0000115>Ein Gebirgssee auf der Turracher Hohe an der Landesgrenze zwischen Karnten und der Steiermark.</obo:IAO_0000115>
        <oboInOwl:hasOBONamespace>GAZ</oboInOwl:hasOBONamespace>
        <oboInOwl:id>GAZ:00103572</oboInOwl:id>
        <rdfs:label>Turracher See</rdfs:label>
    </owl:NamedIndividual>
    


    <!-- http://purl.obolibrary.org/obo/GAZ_00103573 -->

    <owl:NamedIndividual rdf:about="http://purl.obolibrary.org/obo/GAZ_00103573">
        <obo:RO_0001025 rdf:resource="http://purl.obolibrary.org/obo/GAZ_00060626"/>
        <obo:IAO_0000115>A mountain pass situated in the Nock mountains, the western part of the Gurktaler Alps. The area extends from the peaks of the Rinsennock (2,334 m) in the west to the Lattersteighohe (2,264 m) in the east; in the north-south direction, it extends from the village of Turrach to the plain of Reichenau in the south.</obo:IAO_0000115>
        <oboInOwl:hasOBONamespace>GAZ</oboInOwl:hasOBONamespace>
        <oboInOwl:id>GAZ:00103573</oboInOwl:id>
        <rdfs:label>Turracherhohe</rdfs:label>
    </owl:NamedIndividual>
    


    <!-- http://purl.obolibrary.org/obo/GAZ_00103578 -->

    <owl:NamedIndividual rdf:about="http://purl.obolibrary.org/obo/GAZ_00103578">
        <obo:RO_0001025 rdf:resource="http://purl.obolibrary.org/obo/GAZ_00060637"/>
        <obo:IAO_0000115>A lake.</obo:IAO_0000115>
        <oboInOwl:hasOBONamespace>GAZ</oboInOwl:hasOBONamespace>
        <oboInOwl:id>GAZ:00103578</oboInOwl:id>
        <rdfs:label>Hubertussee</rdfs:label>
    </owl:NamedIndividual>
    


    <!-- http://purl.obolibrary.org/obo/GAZ_00103579 -->

    <owl:NamedIndividual rdf:about="http://purl.obolibrary.org/obo/GAZ_00103579">
        <obo:RO_0001025 rdf:resource="http://purl.obolibrary.org/obo/GAZ_00103580"/>
        <obo:IAO_0000115>A lake.</obo:IAO_0000115>
        <oboInOwl:hasOBONamespace>GAZ</oboInOwl:hasOBONamespace>
        <oboInOwl:id>GAZ:00103579</oboInOwl:id>
        <rdfs:label>Ingeringsee</rdfs:label>
    </owl:NamedIndividual>
    


    <!-- http://purl.obolibrary.org/obo/GAZ_00103580 -->

    <owl:NamedIndividual rdf:about="http://purl.obolibrary.org/obo/GAZ_00103580">
        <obo:RO_0001025 rdf:resource="http://purl.obolibrary.org/obo/GAZ_00056786"/>
        <obo:IAO_0000115>Eine kleine Untergruppe der Niederen Tauern in den Zentralalpen der osterreichischen Ostalpen.</obo:IAO_0000115>
        <oboInOwl:hasOBONamespace>GAZ</oboInOwl:hasOBONamespace>
        <oboInOwl:id>GAZ:00103580</oboInOwl:id>
        <rdfs:label>Seckauer Tauern</rdfs:label>
    </owl:NamedIndividual>
    


    <!-- http://purl.obolibrary.org/obo/GAZ_00103581 -->

    <owl:NamedIndividual rdf:about="http://purl.obolibrary.org/obo/GAZ_00103581">
        <obo:RO_0001025 rdf:resource="http://purl.obolibrary.org/obo/GAZ_00056786"/>
        <obo:IAO_0000115>Eine Untergruppe der Zentralalpen in den Ostalpen.</obo:IAO_0000115>
        <oboInOwl:hasOBONamespace>GAZ</oboInOwl:hasOBONamespace>
        <oboInOwl:id>GAZ:00103581</oboInOwl:id>
        <rdfs:label>Rottenmanner und Wolzer Tauern</rdfs:label>
    </owl:NamedIndividual>
    


    <!-- http://purl.obolibrary.org/obo/GAZ_00103582 -->

    <owl:NamedIndividual rdf:about="http://purl.obolibrary.org/obo/GAZ_00103582">
        <obo:RO_0001025 rdf:resource="http://purl.obolibrary.org/obo/GAZ_00056786"/>
        <obo:IAO_0000115>Eine Untergruppe der Zentralalpen in den osterreichischen Ostalpen.</obo:IAO_0000115>
        <oboInOwl:hasOBONamespace>GAZ</oboInOwl:hasOBONamespace>
        <oboInOwl:id>GAZ:00103582</oboInOwl:id>
        <rdfs:label>Radstadter Tauern</rdfs:label>
    </owl:NamedIndividual>
    


    <!-- http://purl.obolibrary.org/obo/GAZ_00103583 -->

    <owl:NamedIndividual rdf:about="http://purl.obolibrary.org/obo/GAZ_00103583">
        <obo:RO_0001025 rdf:resource="http://purl.obolibrary.org/obo/GAZ_00056798"/>
        <obo:IAO_0000115>A lake.</obo:IAO_0000115>
        <oboInOwl:hasOBONamespace>GAZ</oboInOwl:hasOBONamespace>
        <oboInOwl:id>GAZ:00103583</oboInOwl:id>
        <rdfs:label>Kammersee</rdfs:label>
    </owl:NamedIndividual>
    


    <!-- http://purl.obolibrary.org/obo/GAZ_00103617 -->

    <owl:NamedIndividual rdf:about="http://purl.obolibrary.org/obo/GAZ_00103617">
        <obo:RO_0001025 rdf:resource="http://purl.obolibrary.org/obo/GAZ_00060641"/>
        <obo:IAO_0000115>A strongly karstic Austrian mountain, and the second highest mountain in the Northern Limestone Alps. It is situated at the border of Upper Austria and Styria in central Austria, and is the highest point in each of those states. Parts of the massif also lie in the State of Salzburg.</obo:IAO_0000115>
        <oboInOwl:hasOBONamespace>GAZ</oboInOwl:hasOBONamespace>
        <oboInOwl:id>GAZ:00103617</oboInOwl:id>
        <rdfs:label>Hoher Dachstein</rdfs:label>
    </owl:NamedIndividual>
    


    <!-- http://purl.obolibrary.org/obo/GAZ_00103618 -->

    <owl:NamedIndividual rdf:about="http://purl.obolibrary.org/obo/GAZ_00103618">
        <obo:RO_0001025 rdf:resource="http://purl.obolibrary.org/obo/GAZ_00103617"/>
        <obo:IAO_0000115>A karst cave.</obo:IAO_0000115>
        <oboInOwl:hasOBONamespace>GAZ</oboInOwl:hasOBONamespace>
        <oboInOwl:id>GAZ:00103618</oboInOwl:id>
        <rdfs:label>Mammuthhohle</rdfs:label>
    </owl:NamedIndividual>
    


    <!-- http://purl.obolibrary.org/obo/GAZ_00103619 -->

    <owl:NamedIndividual rdf:about="http://purl.obolibrary.org/obo/GAZ_00103619">
        <obo:RO_0001025 rdf:resource="http://purl.obolibrary.org/obo/GAZ_00103617"/>
        <obo:IAO_0000115>A karst cave.</obo:IAO_0000115>
        <oboInOwl:hasOBONamespace>GAZ</oboInOwl:hasOBONamespace>
        <oboInOwl:id>GAZ:00103619</oboInOwl:id>
        <rdfs:label>Hirlatzhohle</rdfs:label>
    </owl:NamedIndividual>
    


    <!-- http://purl.obolibrary.org/obo/GAZ_00143923 -->

    <owl:NamedIndividual rdf:about="http://purl.obolibrary.org/obo/GAZ_00143923">
        <obo:RO_0001025 rdf:resource="http://purl.obolibrary.org/obo/GAZ_00143924"/>
        <obo:IAO_0000115>A 6 km long glacier (2005) situated in the Pennine Alps near the Allalinhorn in the canton of Valais in Switzerland. The glacier is bordered on the west by the Allalinhorn, Rimpfischhorn and Strahlhorn.</obo:IAO_0000115>
        <oboInOwl:hasOBONamespace>GAZ</oboInOwl:hasOBONamespace>
        <oboInOwl:id>GAZ:00143923</oboInOwl:id>
        <rdfs:label>Allalin Glacier</rdfs:label>
    </owl:NamedIndividual>
    


    <!-- http://purl.obolibrary.org/obo/GAZ_00143924 -->

    <owl:NamedIndividual rdf:about="http://purl.obolibrary.org/obo/GAZ_00143924">
        <obo:RO_0001025 rdf:resource="http://purl.obolibrary.org/obo/GAZ_00008403"/>
        <obo:IAO_0000115>A massif in the Pennine Alps of Valais, Switzerland, A which forms the divide between the Saastal and Mattertal.</obo:IAO_0000115>
        <oboInOwl:hasOBONamespace>GAZ</oboInOwl:hasOBONamespace>
        <oboInOwl:id>GAZ:00143924</oboInOwl:id>
        <rdfs:label>Mischabelhorner</rdfs:label>
    </owl:NamedIndividual>
    


    <!-- http://purl.obolibrary.org/obo/GAZ_00143925 -->

    <owl:NamedIndividual rdf:about="http://purl.obolibrary.org/obo/GAZ_00143925">
        <obo:RO_0001025 rdf:resource="http://purl.obolibrary.org/obo/GAZ_00143924"/>
        <obo:IAO_0000115>A glacier in the Mischabelhorner.</obo:IAO_0000115>
        <oboInOwl:hasOBONamespace>GAZ</oboInOwl:hasOBONamespace>
        <oboInOwl:id>GAZ:00143925</oboInOwl:id>
        <rdfs:label>Hohlaub Glaceier</rdfs:label>
    </owl:NamedIndividual>
    


    <!-- http://purl.obolibrary.org/obo/GAZ_00143926 -->

    <owl:NamedIndividual rdf:about="http://purl.obolibrary.org/obo/GAZ_00143926">
        <obo:RO_0001025 rdf:resource="http://purl.obolibrary.org/obo/GAZ_00143924"/>
        <obo:IAO_0000115>A glacier in the Mischabelhorner.</obo:IAO_0000115>
        <oboInOwl:hasOBONamespace>GAZ</oboInOwl:hasOBONamespace>
        <oboInOwl:id>GAZ:00143926</oboInOwl:id>
        <rdfs:label>Ried Glacier</rdfs:label>
    </owl:NamedIndividual>
    


    <!-- http://purl.obolibrary.org/obo/GAZ_00143927 -->

    <owl:NamedIndividual rdf:about="http://purl.obolibrary.org/obo/GAZ_00143927">
        <obo:RO_0001025 rdf:resource="http://purl.obolibrary.org/obo/GAZ_00143924"/>
        <obo:IAO_0000115>A 4.7 km long glacier (2005) situated in the Pennine Alps in the canton of Valais in Switzerland.</obo:IAO_0000115>
        <oboInOwl:hasOBONamespace>GAZ</oboInOwl:hasOBONamespace>
        <oboInOwl:id>GAZ:00143927</oboInOwl:id>
        <rdfs:label>Fee Glacier</rdfs:label>
    </owl:NamedIndividual>
    


    <!-- http://purl.obolibrary.org/obo/GAZ_00143928 -->

    <owl:NamedIndividual rdf:about="http://purl.obolibrary.org/obo/GAZ_00143928">
        <obo:RO_0001025 rdf:resource="http://purl.obolibrary.org/obo/GAZ_00143924"/>
        <obo:IAO_0000115>A glacier in the Mischabelhorner.</obo:IAO_0000115>
        <oboInOwl:hasOBONamespace>GAZ</oboInOwl:hasOBONamespace>
        <oboInOwl:id>GAZ:00143928</oboInOwl:id>
        <rdfs:label>Mellich Glacier</rdfs:label>
    </owl:NamedIndividual>
    


    <!-- http://purl.obolibrary.org/obo/GAZ_00143929 -->

    <owl:NamedIndividual rdf:about="http://purl.obolibrary.org/obo/GAZ_00143929">
        <obo:RO_0001025 rdf:resource="http://purl.obolibrary.org/obo/GAZ_00008403"/>
        <obo:IAO_0000115>A massif in the western Pennine Alps in Switzerland.</obo:IAO_0000115>
        <oboInOwl:hasOBONamespace>GAZ</oboInOwl:hasOBONamespace>
        <oboInOwl:id>GAZ:00143929</oboInOwl:id>
        <rdfs:label>Grand Combin</rdfs:label>
    </owl:NamedIndividual>
    


    <!-- http://purl.obolibrary.org/obo/GAZ_00143930 -->

    <owl:NamedIndividual rdf:about="http://purl.obolibrary.org/obo/GAZ_00143930">
        <obo:RO_0001025 rdf:resource="http://purl.obolibrary.org/obo/GAZ_00143929"/>
        <obo:IAO_0000115>A valley glacier in the Grand Combin massif in the Pennine Alps in southwestern Valais. It is 9.8 km long with an average width of slightly more than 1 km and covers an area of 17.4 km2.</obo:IAO_0000115>
        <oboInOwl:hasOBONamespace>GAZ</oboInOwl:hasOBONamespace>
        <oboInOwl:id>GAZ:00143930</oboInOwl:id>
        <rdfs:label>Corbassiere Glacier</rdfs:label>
    </owl:NamedIndividual>
    


    <!-- http://purl.obolibrary.org/obo/GAZ_00143931 -->

    <owl:NamedIndividual rdf:about="http://purl.obolibrary.org/obo/GAZ_00143931">
        <obo:RO_0001025 rdf:resource="http://purl.obolibrary.org/obo/GAZ_00008403"/>
        <obo:IAO_0000115>A 6.5 km long glacier (2005) situated in the Pennine Alps in the canton of Valais in Switzerland.</obo:IAO_0000115>
        <oboInOwl:hasOBONamespace>GAZ</oboInOwl:hasOBONamespace>
        <oboInOwl:id>GAZ:00143931</oboInOwl:id>
        <rdfs:label>Ferpecle Glacier</rdfs:label>
    </owl:NamedIndividual>
    


    <!-- http://purl.obolibrary.org/obo/GAZ_00143932 -->

    <owl:NamedIndividual rdf:about="http://purl.obolibrary.org/obo/GAZ_00143932">
        <obo:RO_0001025 rdf:resource="http://purl.obolibrary.org/obo/GAZ_00009676"/>
        <obo:IAO_0000115>A valley glacier on the south side of the Bernese Alps in the canton of Valais, Switzerland. The starting point of the Fiescher Glacier is 4000 m above sea level, on the eastern slope of the Fiescherhorn, it is flanked to the west by the Grunhorn and Gross Wannenhorn and to the east by the Finsteraarhorn. In the lower section, the Fiescher Glacier flows south through a deep valley between the Gross Wannenhorn and the Wasenhorn.</obo:IAO_0000115>
        <oboInOwl:hasOBONamespace>GAZ</oboInOwl:hasOBONamespace>
        <oboInOwl:id>GAZ:00143932</oboInOwl:id>
        <rdfs:label>Fiescher Glacier</rdfs:label>
    </owl:NamedIndividual>
    


    <!-- http://purl.obolibrary.org/obo/GAZ_00143933 -->

    <owl:NamedIndividual rdf:about="http://purl.obolibrary.org/obo/GAZ_00143933">
        <obo:RO_0001025 rdf:resource="http://purl.obolibrary.org/obo/GAZ_00008403"/>
        <obo:IAO_0000115>A mountain massif in the Pennine Alps.</obo:IAO_0000115>
        <oboInOwl:hasOBONamespace>GAZ</oboInOwl:hasOBONamespace>
        <oboInOwl:id>GAZ:00143933</oboInOwl:id>
        <rdfs:label>Monte Rosa</rdfs:label>
    </owl:NamedIndividual>
    


    <!-- http://purl.obolibrary.org/obo/GAZ_00143934 -->

    <owl:NamedIndividual rdf:about="http://purl.obolibrary.org/obo/GAZ_00143934">
        <obo:RO_0001025 rdf:resource="http://purl.obolibrary.org/obo/GAZ_00143933"/>
        <obo:IAO_0000115>A valley glacier found on the Monte Rosa massif close to Zermatt in the canton of Valais, Switzerland. It is about 14 km long and 1 to 1.5 km wide.</obo:IAO_0000115>
        <oboInOwl:hasOBONamespace>GAZ</oboInOwl:hasOBONamespace>
        <oboInOwl:id>GAZ:00143934</oboInOwl:id>
        <rdfs:label>Gorner Glacier</rdfs:label>
    </owl:NamedIndividual>
    


    <!-- http://purl.obolibrary.org/obo/GAZ_00143935 -->

    <owl:NamedIndividual rdf:about="http://purl.obolibrary.org/obo/GAZ_00143935">
        <obo:RO_0001025 rdf:resource="http://purl.obolibrary.org/obo/GAZ_00143933"/>
        <obo:IAO_0000115>A valley glacier in the Monte Rosa massif east of Zermatt in the Pennine Alps. The starting point of the Findel Glacier is on the Cima di Jazzi at 3803 m above sea level, on the border between Switzerland and Italy. From there the glacier flows to the west between the Rimpfischhorn and Strahlhorn on the north and the Stockhorn on the south.</obo:IAO_0000115>
        <oboInOwl:hasOBONamespace>GAZ</oboInOwl:hasOBONamespace>
        <oboInOwl:id>GAZ:00143935</oboInOwl:id>
        <rdfs:label>Findel Glacier</rdfs:label>
    </owl:NamedIndividual>
    


    <!-- http://purl.obolibrary.org/obo/GAZ_00143936 -->

    <owl:NamedIndividual rdf:about="http://purl.obolibrary.org/obo/GAZ_00143936">
        <obo:RO_0001025 rdf:resource="http://purl.obolibrary.org/obo/GAZ_00009676"/>
        <obo:IAO_0000115>A 6.2 km long glacier (2005) situated in the Bernese Alps in the canton of Berne in Switzerland.</obo:IAO_0000115>
        <oboInOwl:hasOBONamespace>GAZ</oboInOwl:hasOBONamespace>
        <oboInOwl:id>GAZ:00143936</oboInOwl:id>
        <rdfs:label>Gauli Glacier</rdfs:label>
    </owl:NamedIndividual>
    


    <!-- http://purl.obolibrary.org/obo/GAZ_00143937 -->

    <owl:NamedIndividual rdf:about="http://purl.obolibrary.org/obo/GAZ_00143937">
        <obo:RO_0001025 rdf:resource="http://purl.obolibrary.org/obo/GAZ_00009676"/>
        <obo:IAO_0000115>The largest glacier in the Alps, covers more than 120 km2 in southern Switzerland. It descends round the south of the Jungfrau into the valley of the Upper Rhone; at its eastern extremity lies a glacier lake, Lake Merjelen (2,350 m). To the west rises Aletschhorn (4,195 m).</obo:IAO_0000115>
        <oboInOwl:hasOBONamespace>GAZ</oboInOwl:hasOBONamespace>
        <oboInOwl:id>GAZ:00143937</oboInOwl:id>
        <rdfs:label>Aletsch Glacier</rdfs:label>
    </owl:NamedIndividual>
    


    <!-- http://purl.obolibrary.org/obo/GAZ_00143938 -->

    <owl:NamedIndividual rdf:about="http://purl.obolibrary.org/obo/GAZ_00143938">
        <obo:RO_0001025 rdf:resource="http://purl.obolibrary.org/obo/GAZ_00009674"/>
        <obo:IAO_0000115>A 7 km long glacier (2005) situated in the Glarus Alps in the canton of Uri in Switzerland.</obo:IAO_0000115>
        <oboInOwl:hasOBONamespace>GAZ</oboInOwl:hasOBONamespace>
        <oboInOwl:id>GAZ:00143938</oboInOwl:id>
        <rdfs:label>Hufi Glacier</rdfs:label>
    </owl:NamedIndividual>
    


    <!-- http://purl.obolibrary.org/obo/GAZ_00143939 -->

    <owl:NamedIndividual rdf:about="http://purl.obolibrary.org/obo/GAZ_00143939">
        <obo:RO_0001025 rdf:resource="http://purl.obolibrary.org/obo/GAZ_00009674"/>
        <obo:IAO_0000115>A 4 km long glacier (2005) situated in the Glarus Alps in the canton of Glarus in Switzerland.</obo:IAO_0000115>
        <oboInOwl:hasOBONamespace>GAZ</oboInOwl:hasOBONamespace>
        <oboInOwl:id>GAZ:00143939</oboInOwl:id>
        <rdfs:label>Biferten Glacier</rdfs:label>
    </owl:NamedIndividual>
    


    <!-- http://purl.obolibrary.org/obo/GAZ_00143940 -->

    <owl:NamedIndividual rdf:about="http://purl.obolibrary.org/obo/GAZ_00143940">
        <obo:RO_0001025 rdf:resource="http://purl.obolibrary.org/obo/GAZ_00009674"/>
        <obo:IAO_0000115>A 2 km long glacier (2005) situated in the Glarus Alps in the cantons of Glarus and Graubunden in Switzerland.</obo:IAO_0000115>
        <oboInOwl:hasOBONamespace>GAZ</oboInOwl:hasOBONamespace>
        <oboInOwl:id>GAZ:00143940</oboInOwl:id>
        <rdfs:label>Vorab Glacier</rdfs:label>
    </owl:NamedIndividual>
    


    <!-- http://purl.obolibrary.org/obo/GAZ_00143941 -->

    <owl:NamedIndividual rdf:about="http://purl.obolibrary.org/obo/GAZ_00143941">
        <obo:RO_0001025 rdf:resource="http://purl.obolibrary.org/obo/GAZ_00009674"/>
        <obo:IAO_0000115>A 3 km long glacier (2005) situated in the Glarus Alps in the canton of Glarus in Switzerland.</obo:IAO_0000115>
        <oboInOwl:hasOBONamespace>GAZ</oboInOwl:hasOBONamespace>
        <oboInOwl:id>GAZ:00143941</oboInOwl:id>
        <rdfs:label>Limmern Glacier</rdfs:label>
    </owl:NamedIndividual>
    


    <!-- http://purl.obolibrary.org/obo/GAZ_00143942 -->

    <owl:NamedIndividual rdf:about="http://purl.obolibrary.org/obo/GAZ_00143942">
        <obo:RO_0001025 rdf:resource="http://purl.obolibrary.org/obo/GAZ_00009676"/>
        <obo:IAO_0000115>A 6.6 km long glacier (2005) situated in the Bernese Alps in the canton of Berne in Switzerland.</obo:IAO_0000115>
        <oboInOwl:hasOBONamespace>GAZ</oboInOwl:hasOBONamespace>
        <oboInOwl:id>GAZ:00143942</oboInOwl:id>
        <rdfs:label>Kander Glacier</rdfs:label>
    </owl:NamedIndividual>
    


    <!-- http://purl.obolibrary.org/obo/GAZ_00143943 -->

    <owl:NamedIndividual rdf:about="http://purl.obolibrary.org/obo/GAZ_00143943">
        <obo:RO_0001025 rdf:resource="http://purl.obolibrary.org/obo/GAZ_00009676"/>
        <obo:IAO_0000115>A 6.6 km long glacier (2005) situated in the Bernese Alps in the canton of Valais in Switzerland.</obo:IAO_0000115>
        <oboInOwl:hasOBONamespace>GAZ</oboInOwl:hasOBONamespace>
        <oboInOwl:id>GAZ:00143943</oboInOwl:id>
        <rdfs:label>Lang Glacier</rdfs:label>
    </owl:NamedIndividual>
    


    <!-- http://purl.obolibrary.org/obo/GAZ_00143944 -->

    <owl:NamedIndividual rdf:about="http://purl.obolibrary.org/obo/GAZ_00143944">
        <obo:RO_0001025 rdf:resource="http://purl.obolibrary.org/obo/GAZ_00008403"/>
        <obo:IAO_0000115>A 7.9 km long glacier (2005) situated in the Pennine Alps in the canton of Valais in Switzerland.</obo:IAO_0000115>
        <oboInOwl:hasOBONamespace>GAZ</oboInOwl:hasOBONamespace>
        <oboInOwl:id>GAZ:00143944</oboInOwl:id>
        <rdfs:label>Mont Mine Glacier</rdfs:label>
    </owl:NamedIndividual>
    


    <!-- http://purl.obolibrary.org/obo/GAZ_00143945 -->

    <owl:NamedIndividual rdf:about="http://purl.obolibrary.org/obo/GAZ_00143945">
        <obo:RO_0001025 rdf:resource="http://purl.obolibrary.org/obo/GAZ_00057287"/>
        <obo:IAO_0000115>A 4 km long glacier (2005) situated in the Bernina Range in the canton of Graubunden in Switzerland.</obo:IAO_0000115>
        <oboInOwl:hasOBONamespace>GAZ</oboInOwl:hasOBONamespace>
        <oboInOwl:id>GAZ:00143945</oboInOwl:id>
        <rdfs:label>Roseg Glacier</rdfs:label>
    </owl:NamedIndividual>
    


    <!-- http://purl.obolibrary.org/obo/GAZ_00143946 -->

    <owl:NamedIndividual rdf:about="http://purl.obolibrary.org/obo/GAZ_00143946">
        <obo:RO_0001025 rdf:resource="http://purl.obolibrary.org/obo/GAZ_00057287"/>
        <obo:IAO_0000115>A 4 km long glacier (2005) situated in the Bernina Range in the canton of Graubunden in Switzerland.</obo:IAO_0000115>
        <oboInOwl:hasOBONamespace>GAZ</oboInOwl:hasOBONamespace>
        <oboInOwl:id>GAZ:00143946</oboInOwl:id>
        <rdfs:label>Tschierva Glacier</rdfs:label>
    </owl:NamedIndividual>
    


    <!-- http://purl.obolibrary.org/obo/GAZ_00143947 -->

    <owl:NamedIndividual rdf:about="http://purl.obolibrary.org/obo/GAZ_00143947">
        <obo:RO_0001025 rdf:resource="http://purl.obolibrary.org/obo/GAZ_00057287"/>
        <obo:IAO_0000115>A valley glacier.</obo:IAO_0000115>
        <oboInOwl:hasOBONamespace>GAZ</oboInOwl:hasOBONamespace>
        <oboInOwl:id>GAZ:00143947</oboInOwl:id>
        <rdfs:label>Morteratsch Glacier</rdfs:label>
    </owl:NamedIndividual>
    


    <!-- http://purl.obolibrary.org/obo/GAZ_00143948 -->

    <owl:NamedIndividual rdf:about="http://purl.obolibrary.org/obo/GAZ_00143948">
        <obo:RO_0001025 rdf:resource="http://purl.obolibrary.org/obo/GAZ_00057287"/>
        <obo:IAO_0000115>A 3.5 km long glacier (2005) situated in the Bernina Range in the canton of Graubunden in Switzerland.</obo:IAO_0000115>
        <oboInOwl:hasOBONamespace>GAZ</oboInOwl:hasOBONamespace>
        <oboInOwl:id>GAZ:00143948</oboInOwl:id>
        <rdfs:label>Palu Glacier</rdfs:label>
    </owl:NamedIndividual>
    


    <!-- http://purl.obolibrary.org/obo/GAZ_00143949 -->

    <owl:NamedIndividual rdf:about="http://purl.obolibrary.org/obo/GAZ_00143949">
        <obo:RO_0001025 rdf:resource="http://purl.obolibrary.org/obo/GAZ_00009676"/>
        <obo:IAO_0000115>A valley glacier on the south side of the Bernese Alps, in the canton of Valais.</obo:IAO_0000115>
        <oboInOwl:hasOBONamespace>GAZ</oboInOwl:hasOBONamespace>
        <oboInOwl:id>GAZ:00143949</oboInOwl:id>
        <rdfs:label>Oberaletsch Glacier</rdfs:label>
    </owl:NamedIndividual>
    


    <!-- http://purl.obolibrary.org/obo/GAZ_00143950 -->

    <owl:NamedIndividual rdf:about="http://purl.obolibrary.org/obo/GAZ_00143950">
        <obo:RO_0001025 rdf:resource="http://purl.obolibrary.org/obo/GAZ_00009676"/>
        <obo:IAO_0000115>One of the two valley glaciers north of Grindelwald on the northern side of the Bernese Alps, in the Canton of Berne. The Upper Grindelwald Glacier arises from a vast snow field south of Schreckhorn and north of Wetterhorn.</obo:IAO_0000115>
        <oboInOwl:hasOBONamespace>GAZ</oboInOwl:hasOBONamespace>
        <oboInOwl:id>GAZ:00143950</oboInOwl:id>
        <rdfs:label>Upper Grindelwald Glacier</rdfs:label>
    </owl:NamedIndividual>
    


    <!-- http://purl.obolibrary.org/obo/GAZ_00143951 -->

    <owl:NamedIndividual rdf:about="http://purl.obolibrary.org/obo/GAZ_00143951">
        <obo:RO_0001025 rdf:resource="http://purl.obolibrary.org/obo/GAZ_00009676"/>
        <obo:IAO_0000115>The western one of the two Grindelwald Glaciers in the Bernese Alps, north of Grindelwald.</obo:IAO_0000115>
        <oboInOwl:hasOBONamespace>GAZ</oboInOwl:hasOBONamespace>
        <oboInOwl:id>GAZ:00143951</oboInOwl:id>
        <rdfs:label>Lower Grindelwald Glacier</rdfs:label>
    </owl:NamedIndividual>
    


    <!-- http://purl.obolibrary.org/obo/GAZ_00143952 -->

    <owl:NamedIndividual rdf:about="http://purl.obolibrary.org/obo/GAZ_00143952">
        <obo:RO_0001025 rdf:resource="http://purl.obolibrary.org/obo/GAZ_00056810"/>
        <obo:IAO_0000115>A 5 km long glacier (2005) situated in the Urner Alps in the canton of Berne in Switzerland.</obo:IAO_0000115>
        <oboInOwl:hasOBONamespace>GAZ</oboInOwl:hasOBONamespace>
        <oboInOwl:id>GAZ:00143952</oboInOwl:id>
        <rdfs:label>Trift Glacier</rdfs:label>
    </owl:NamedIndividual>
    


    <!-- http://purl.obolibrary.org/obo/GAZ_00143953 -->

    <owl:NamedIndividual rdf:about="http://purl.obolibrary.org/obo/GAZ_00143953">
        <obo:RO_0001025 rdf:resource="http://purl.obolibrary.org/obo/GAZ_00008403"/>
        <obo:IAO_0000115>A 7.7 km long glacier (2005) situated in the Pennine Alps in the canton of Valais in Switzerland.</obo:IAO_0000115>
        <oboInOwl:hasOBONamespace>GAZ</oboInOwl:hasOBONamespace>
        <oboInOwl:id>GAZ:00143953</oboInOwl:id>
        <rdfs:label>Otemma Glacier</rdfs:label>
    </owl:NamedIndividual>
    


    <!-- http://purl.obolibrary.org/obo/GAZ_00143954 -->

    <owl:NamedIndividual rdf:about="http://purl.obolibrary.org/obo/GAZ_00143954">
        <obo:RO_0001025 rdf:resource="http://purl.obolibrary.org/obo/GAZ_00056810"/>
        <obo:IAO_0000115>The glacier that is the source of the Rhone River and one of the primary contributors to Lake Geneva in the far eastern end of the canton of Valais in Switzerland. It is located in the Urner Alps near the Grimsel Pass, and is part of the Oberwald municipality.</obo:IAO_0000115>
        <oboInOwl:hasOBONamespace>GAZ</oboInOwl:hasOBONamespace>
        <oboInOwl:id>GAZ:00143954</oboInOwl:id>
        <rdfs:label>Rhone Glacier</rdfs:label>
    </owl:NamedIndividual>
    


    <!-- http://purl.obolibrary.org/obo/GAZ_00143955 -->

    <owl:NamedIndividual rdf:about="http://purl.obolibrary.org/obo/GAZ_00143955">
        <obo:RO_0001025 rdf:resource="http://purl.obolibrary.org/obo/GAZ_00060584"/>
        <obo:IAO_0000115>A 6.3 km long glacier (2002) situated in the Mont Blanc Massif in the canton of Valais in Switzerland.</obo:IAO_0000115>
        <oboInOwl:hasOBONamespace>GAZ</oboInOwl:hasOBONamespace>
        <oboInOwl:id>GAZ:00143955</oboInOwl:id>
        <rdfs:label>Glacier de Saleina</rdfs:label>
    </owl:NamedIndividual>
    


    <!-- http://purl.obolibrary.org/obo/GAZ_00143956 -->

    <owl:NamedIndividual rdf:about="http://purl.obolibrary.org/obo/GAZ_00143956">
        <obo:RO_0001025 rdf:resource="http://purl.obolibrary.org/obo/GAZ_00143959"/>
        <obo:IAO_0000115>The largest of the two sources of the Aare river in the Bernese Alps. It emerges from the association of the Finsteraargletscher and the Lauteraargletscher and flows for about 6 km to the east down to the Grimselsee near the Grimsel Pass.</obo:IAO_0000115>
        <oboInOwl:hasOBONamespace>GAZ</oboInOwl:hasOBONamespace>
        <oboInOwl:id>GAZ:00143956</oboInOwl:id>
        <rdfs:label>Unteraar Glacier</rdfs:label>
    </owl:NamedIndividual>
    


    <!-- http://purl.obolibrary.org/obo/GAZ_00143957 -->

    <owl:NamedIndividual rdf:about="http://purl.obolibrary.org/obo/GAZ_00143957">
        <obo:RO_0001025 rdf:resource="http://purl.obolibrary.org/obo/GAZ_00008403"/>
        <obo:IAO_0000115>A 7 km long glacier (2005) situated in the Pennine Alps in the canton of Valais in Switzerland.</obo:IAO_0000115>
        <oboInOwl:hasOBONamespace>GAZ</oboInOwl:hasOBONamespace>
        <oboInOwl:id>GAZ:00143957</oboInOwl:id>
        <rdfs:label>Zinal Glacier</rdfs:label>
    </owl:NamedIndividual>
    


    <!-- http://purl.obolibrary.org/obo/GAZ_00143958 -->

    <owl:NamedIndividual rdf:about="http://purl.obolibrary.org/obo/GAZ_00143958">
        <obo:RO_0001025 rdf:resource="http://purl.obolibrary.org/obo/GAZ_00008403"/>
        <obo:IAO_0000115>A 6 km long glacier (2005) situated in the Pennine Alps in the canton of Valais in Switzerland.</obo:IAO_0000115>
        <oboInOwl:hasOBONamespace>GAZ</oboInOwl:hasOBONamespace>
        <oboInOwl:id>GAZ:00143958</oboInOwl:id>
        <rdfs:label>Zmutt Glacier</rdfs:label>
    </owl:NamedIndividual>
    


    <!-- http://purl.obolibrary.org/obo/GAZ_00143959 -->

    <owl:NamedIndividual rdf:about="http://purl.obolibrary.org/obo/GAZ_00143959">
        <obo:RO_0001025 rdf:resource="http://purl.obolibrary.org/obo/GAZ_00009676"/>
        <obo:IAO_0000115>Glaciers located at the sources of the Aar River in the Bernese Alps, Switzerland.</obo:IAO_0000115>
        <oboInOwl:hasOBONamespace>GAZ</oboInOwl:hasOBONamespace>
        <oboInOwl:id>GAZ:00143959</oboInOwl:id>
        <rdfs:label>Aar Glaciers</rdfs:label>
    </owl:NamedIndividual>
    


    <!-- http://purl.obolibrary.org/obo/GAZ_00143960 -->

    <owl:NamedIndividual rdf:about="http://purl.obolibrary.org/obo/GAZ_00143960">
        <obo:RO_0001025 rdf:resource="http://purl.obolibrary.org/obo/GAZ_00143956"/>
        <oboInOwl:hasOBONamespace>GAZ</oboInOwl:hasOBONamespace>
        <oboInOwl:id>GAZ:00143960</oboInOwl:id>
        <rdfs:label>Lauteraar Glacier</rdfs:label>
    </owl:NamedIndividual>
    


    <!-- http://purl.obolibrary.org/obo/GAZ_00143961 -->

    <owl:NamedIndividual rdf:about="http://purl.obolibrary.org/obo/GAZ_00143961">
        <obo:RO_0001025 rdf:resource="http://purl.obolibrary.org/obo/GAZ_00143956"/>
        <oboInOwl:hasOBONamespace>GAZ</oboInOwl:hasOBONamespace>
        <oboInOwl:id>GAZ:00143961</oboInOwl:id>
        <rdfs:label>Finsteraar Glacier</rdfs:label>
    </owl:NamedIndividual>
    


    <!-- http://purl.obolibrary.org/obo/GAZ_00143962 -->

    <owl:NamedIndividual rdf:about="http://purl.obolibrary.org/obo/GAZ_00143962">
        <obo:RO_0001025 rdf:resource="http://purl.obolibrary.org/obo/GAZ_00143959"/>
        <obo:IAO_0000115>A 4 km long glacier (2005) situated in the Bernese Alps in the canton of Berne in Switzerland.</obo:IAO_0000115>
        <oboInOwl:hasOBONamespace>GAZ</oboInOwl:hasOBONamespace>
        <oboInOwl:id>GAZ:00143962</oboInOwl:id>
        <rdfs:label>Oberaar Glacier</rdfs:label>
    </owl:NamedIndividual>
    


    <!-- http://purl.obolibrary.org/obo/GAZ_00143963 -->

    <owl:NamedIndividual rdf:about="http://purl.obolibrary.org/obo/GAZ_00143963">
        <obo:RO_0001025 rdf:resource="http://purl.obolibrary.org/obo/GAZ_00057288"/>
        <obo:IAO_0000115>A 3.5 km long glacier (2005) situated in the Bregaglia Range in the canton of Graubunden in Switzerland.</obo:IAO_0000115>
        <oboInOwl:hasOBONamespace>GAZ</oboInOwl:hasOBONamespace>
        <oboInOwl:id>GAZ:00143963</oboInOwl:id>
        <rdfs:label>Albigna Glacier</rdfs:label>
    </owl:NamedIndividual>
    


    <!-- http://purl.obolibrary.org/obo/GAZ_00143964 -->

    <owl:NamedIndividual rdf:about="http://purl.obolibrary.org/obo/GAZ_00143964">
        <obo:RO_0001025 rdf:resource="http://purl.obolibrary.org/obo/GAZ_00008403"/>
        <obo:IAO_0000115>A 4 km long glacier (2005) situated in the Pennine Alps in the canton of Valais in Switzerland.</obo:IAO_0000115>
        <oboInOwl:hasOBONamespace>GAZ</oboInOwl:hasOBONamespace>
        <oboInOwl:id>GAZ:00143964</oboInOwl:id>
        <rdfs:label>Arolla Glacier</rdfs:label>
    </owl:NamedIndividual>
    


    <!-- http://purl.obolibrary.org/obo/GAZ_00143965 -->

    <owl:NamedIndividual rdf:about="http://purl.obolibrary.org/obo/GAZ_00143965">
        <obo:RO_0001025 rdf:resource="http://purl.obolibrary.org/obo/GAZ_00143964"/>
        <obo:IAO_0000115>A component of the Arolla Glacier.</obo:IAO_0000115>
        <oboInOwl:hasOBONamespace>GAZ</oboInOwl:hasOBONamespace>
        <oboInOwl:id>GAZ:00143965</oboInOwl:id>
        <rdfs:label>Glacier du Mont Collon</rdfs:label>
    </owl:NamedIndividual>
    


    <!-- http://purl.obolibrary.org/obo/GAZ_00143966 -->

    <owl:NamedIndividual rdf:about="http://purl.obolibrary.org/obo/GAZ_00143966">
        <obo:RO_0001025 rdf:resource="http://purl.obolibrary.org/obo/GAZ_00143964"/>
        <obo:IAO_0000115>A component of the Arolla Glacier.</obo:IAO_0000115>
        <oboInOwl:hasOBONamespace>GAZ</oboInOwl:hasOBONamespace>
        <oboInOwl:id>GAZ:00143966</oboInOwl:id>
        <rdfs:label>Haut Glacier d&apos;Arolla</rdfs:label>
    </owl:NamedIndividual>
    


    <!-- http://purl.obolibrary.org/obo/GAZ_00143967 -->

    <owl:NamedIndividual rdf:about="http://purl.obolibrary.org/obo/GAZ_00143967">
        <obo:RO_0001025 rdf:resource="http://purl.obolibrary.org/obo/GAZ_00009680"/>
        <obo:IAO_0000115>A 1.5 km long glacier (2005) situated in the Lepontine Alps in the canton of Ticino in Switzerland.</obo:IAO_0000115>
        <oboInOwl:hasOBONamespace>GAZ</oboInOwl:hasOBONamespace>
        <oboInOwl:id>GAZ:00143967</oboInOwl:id>
        <rdfs:label>Basodino Glacier</rdfs:label>
    </owl:NamedIndividual>
    


    <!-- http://purl.obolibrary.org/obo/GAZ_00143968 -->

    <owl:NamedIndividual rdf:about="http://purl.obolibrary.org/obo/GAZ_00143968">
        <obo:RO_0001025 rdf:resource="http://purl.obolibrary.org/obo/GAZ_00008403"/>
        <obo:IAO_0000115>A 2 km long glacier (2005) situated in the Pennine Alps in the canton of Valais in Switzerland.</obo:IAO_0000115>
        <oboInOwl:hasOBONamespace>GAZ</oboInOwl:hasOBONamespace>
        <oboInOwl:id>GAZ:00143968</oboInOwl:id>
        <rdfs:label>Boveire Glacier</rdfs:label>
    </owl:NamedIndividual>
    


    <!-- http://purl.obolibrary.org/obo/GAZ_00143969 -->

    <owl:NamedIndividual rdf:about="http://purl.obolibrary.org/obo/GAZ_00143969">
        <obo:RO_0001025 rdf:resource="http://purl.obolibrary.org/obo/GAZ_00008403"/>
        <obo:IAO_0000115>A 4 km long glacier (2005) situated in the Pennine Alps in the canton of Valais in Switzerland.</obo:IAO_0000115>
        <oboInOwl:hasOBONamespace>GAZ</oboInOwl:hasOBONamespace>
        <oboInOwl:id>GAZ:00143969</oboInOwl:id>
        <rdfs:label>Brunegg Glacier</rdfs:label>
    </owl:NamedIndividual>
    


    <!-- http://purl.obolibrary.org/obo/GAZ_00143970 -->

    <owl:NamedIndividual rdf:about="http://purl.obolibrary.org/obo/GAZ_00143970">
        <obo:RO_0001025 rdf:resource="http://purl.obolibrary.org/obo/GAZ_00008403"/>
        <obo:IAO_0000115>A 3 km long glacier (2005) situated in the Pennine Alps in the canton of Valais in Switzerland.</obo:IAO_0000115>
        <oboInOwl:hasOBONamespace>GAZ</oboInOwl:hasOBONamespace>
        <oboInOwl:id>GAZ:00143970</oboInOwl:id>
        <rdfs:label>Cheilon Glacier</rdfs:label>
    </owl:NamedIndividual>
    


    <!-- http://purl.obolibrary.org/obo/GAZ_00143971 -->

    <owl:NamedIndividual rdf:about="http://purl.obolibrary.org/obo/GAZ_00143971">
        <obo:RO_0001025 rdf:resource="http://purl.obolibrary.org/obo/GAZ_00056810"/>
        <obo:IAO_0000115>A 2.5 km long glacier (2005) situated in the Urner Alps in the canton of Uri in Switzerland.</obo:IAO_0000115>
        <oboInOwl:hasOBONamespace>GAZ</oboInOwl:hasOBONamespace>
        <oboInOwl:id>GAZ:00143971</oboInOwl:id>
        <rdfs:label>Chelen Glacier</rdfs:label>
    </owl:NamedIndividual>
    


    <!-- http://purl.obolibrary.org/obo/GAZ_00143972 -->

    <owl:NamedIndividual rdf:about="http://purl.obolibrary.org/obo/GAZ_00143972">
        <obo:RO_0001025 rdf:resource="http://purl.obolibrary.org/obo/GAZ_00056810"/>
        <obo:IAO_0000115>A 2 km long glacier (2005) situated in the Urner Alps in the canton of Uri in Switzerland.</obo:IAO_0000115>
        <oboInOwl:hasOBONamespace>GAZ</oboInOwl:hasOBONamespace>
        <oboInOwl:id>GAZ:00143972</oboInOwl:id>
        <rdfs:label>Damma Glacier</rdfs:label>
    </owl:NamedIndividual>
    


    <!-- http://purl.obolibrary.org/obo/GAZ_00143973 -->

    <owl:NamedIndividual rdf:about="http://purl.obolibrary.org/obo/GAZ_00143973">
        <obo:RO_0001025 rdf:resource="http://purl.obolibrary.org/obo/GAZ_00009676"/>
        <obo:IAO_0000115>A mountain massif in the Bernese Alps.</obo:IAO_0000115>
        <oboInOwl:hasOBONamespace>GAZ</oboInOwl:hasOBONamespace>
        <oboInOwl:id>GAZ:00143973</oboInOwl:id>
        <rdfs:label>Les Diablerets Massif</rdfs:label>
    </owl:NamedIndividual>
    


    <!-- http://purl.obolibrary.org/obo/GAZ_00143974 -->

    <owl:NamedIndividual rdf:about="http://purl.obolibrary.org/obo/GAZ_00143974">
        <obo:RO_0001025 rdf:resource="http://purl.obolibrary.org/obo/GAZ_00143975"/>
        <obo:IAO_0000115>A glacier situated on the summit of Les Diablerets in the Bernese Alps.</obo:IAO_0000115>
        <oboInOwl:hasOBONamespace>GAZ</oboInOwl:hasOBONamespace>
        <oboInOwl:id>GAZ:00143974</oboInOwl:id>
        <rdfs:label>Diablerets Glacier</rdfs:label>
    </owl:NamedIndividual>
    


    <!-- http://purl.obolibrary.org/obo/GAZ_00143975 -->

    <owl:NamedIndividual rdf:about="http://purl.obolibrary.org/obo/GAZ_00143975">
        <obo:RO_0001025 rdf:resource="http://purl.obolibrary.org/obo/GAZ_00143973"/>
        <obo:IAO_0000115>The summit of Les Diablerets Massif.</obo:IAO_0000115>
        <oboInOwl:hasOBONamespace>GAZ</oboInOwl:hasOBONamespace>
        <oboInOwl:id>GAZ:00143975</oboInOwl:id>
        <rdfs:label>Summit of les Diablerets</rdfs:label>
    </owl:NamedIndividual>
    


    <!-- http://purl.obolibrary.org/obo/GAZ_00143976 -->

    <owl:NamedIndividual rdf:about="http://purl.obolibrary.org/obo/GAZ_00143976">
        <obo:RO_0001025 rdf:resource="http://purl.obolibrary.org/obo/GAZ_00009676"/>
        <obo:IAO_0000115>A 3 km long glacier (2005) situated in the Bernese Alps in the canton of Berne in Switzerland.</obo:IAO_0000115>
        <oboInOwl:hasOBONamespace>GAZ</oboInOwl:hasOBONamespace>
        <oboInOwl:id>GAZ:00143976</oboInOwl:id>
        <rdfs:label>Tschingel Glacier</rdfs:label>
    </owl:NamedIndividual>
    


    <!-- http://purl.obolibrary.org/obo/GAZ_00143977 -->

    <owl:NamedIndividual rdf:about="http://purl.obolibrary.org/obo/GAZ_00143977">
        <obo:RO_0001025 rdf:resource="http://purl.obolibrary.org/obo/GAZ_00008403"/>
        <obo:IAO_0000115>A 2.5 km long glacier (2005) situated in the Pennine Alps in the canton of Valais in Switzerland.</obo:IAO_0000115>
        <oboInOwl:hasOBONamespace>GAZ</oboInOwl:hasOBONamespace>
        <oboInOwl:id>GAZ:00143977</oboInOwl:id>
        <rdfs:label>Eiger Glacier</rdfs:label>
    </owl:NamedIndividual>
    


    <!-- http://purl.obolibrary.org/obo/GAZ_00143978 -->

    <owl:NamedIndividual rdf:about="http://purl.obolibrary.org/obo/GAZ_00143978">
        <obo:RO_0001025 rdf:resource="http://purl.obolibrary.org/obo/GAZ_00057288"/>
        <obo:IAO_0000115>A 6 km long glacier (2005) situated in the Bregaglia Range in the canton of Graubunden in Switzerland.</obo:IAO_0000115>
        <oboInOwl:hasOBONamespace>GAZ</oboInOwl:hasOBONamespace>
        <oboInOwl:id>GAZ:00143978</oboInOwl:id>
        <rdfs:label>Forno Glacier</rdfs:label>
    </owl:NamedIndividual>
    


    <!-- http://purl.obolibrary.org/obo/GAZ_00143979 -->

    <owl:NamedIndividual rdf:about="http://purl.obolibrary.org/obo/GAZ_00143979">
        <obo:RO_0001025 rdf:resource="http://purl.obolibrary.org/obo/GAZ_00008403"/>
        <obo:IAO_0000115>A 4 km long glacier (2005) situated in the Pennine Alps in the canton of Valais in Switzerland.</obo:IAO_0000115>
        <oboInOwl:hasOBONamespace>GAZ</oboInOwl:hasOBONamespace>
        <oboInOwl:id>GAZ:00143979</oboInOwl:id>
        <rdfs:label>Gietro Glacier</rdfs:label>
    </owl:NamedIndividual>
    


    <!-- http://purl.obolibrary.org/obo/GAZ_00143980 -->

    <owl:NamedIndividual rdf:about="http://purl.obolibrary.org/obo/GAZ_00143980">
        <obo:RO_0001025 rdf:resource="http://purl.obolibrary.org/obo/GAZ_00143981"/>
        <obo:IAO_0000115>A glacier in the Glarus Alps.</obo:IAO_0000115>
        <oboInOwl:hasOBONamespace>GAZ</oboInOwl:hasOBONamespace>
        <oboInOwl:id>GAZ:00143980</oboInOwl:id>
        <rdfs:label>Glarnischfirn</rdfs:label>
    </owl:NamedIndividual>
    


    <!-- http://purl.obolibrary.org/obo/GAZ_00143981 -->

    <owl:NamedIndividual rdf:about="http://purl.obolibrary.org/obo/GAZ_00143981">
        <obo:RO_0001025 rdf:resource="http://purl.obolibrary.org/obo/GAZ_00009674"/>
        <obo:IAO_0000115>A mountain of the Glarus Alps, Switzerland, consisting of two ridges of either side of the Glarnischfirn glacier: the Ruchen at 2901 m to the west, rising above the Klontalersee, and the Bachistock at 2914 m to the southwest.</obo:IAO_0000115>
        <oboInOwl:hasOBONamespace>GAZ</oboInOwl:hasOBONamespace>
        <oboInOwl:id>GAZ:00143981</oboInOwl:id>
        <rdfs:label>Glarnisch</rdfs:label>
    </owl:NamedIndividual>
    


    <!-- http://purl.obolibrary.org/obo/GAZ_00143982 -->

    <owl:NamedIndividual rdf:about="http://purl.obolibrary.org/obo/GAZ_00143982">
        <obo:RO_0001025 rdf:resource="http://purl.obolibrary.org/obo/GAZ_00008403"/>
        <obo:IAO_0000115>A mountain in the Pennine Alps.</obo:IAO_0000115>
        <oboInOwl:hasOBONamespace>GAZ</oboInOwl:hasOBONamespace>
        <oboInOwl:id>GAZ:00143982</oboInOwl:id>
        <rdfs:label>Rosablanche</rdfs:label>
    </owl:NamedIndividual>
    


    <!-- http://purl.obolibrary.org/obo/GAZ_00143983 -->

    <owl:NamedIndividual rdf:about="http://purl.obolibrary.org/obo/GAZ_00143983">
        <obo:RO_0001025 rdf:resource="http://purl.obolibrary.org/obo/GAZ_00143982"/>
        <obo:IAO_0000115>A 2 km long glacier (2005) situated on the Rosablanche in the Pennine Alps in the canton of Valais in Switzerland.</obo:IAO_0000115>
        <oboInOwl:hasOBONamespace>GAZ</oboInOwl:hasOBONamespace>
        <oboInOwl:id>GAZ:00143983</oboInOwl:id>
        <rdfs:label>Grand Desert</rdfs:label>
    </owl:NamedIndividual>
    


    <!-- http://purl.obolibrary.org/obo/GAZ_00143984 -->

    <owl:NamedIndividual rdf:about="http://purl.obolibrary.org/obo/GAZ_00143984">
        <obo:RO_0001025 rdf:resource="http://purl.obolibrary.org/obo/GAZ_00057284"/>
        <obo:IAO_0000115>A 2 km long glacier (2005) situated in the Silvretta Range in the canton of Graubunden in Switzerland.</obo:IAO_0000115>
        <oboInOwl:hasOBONamespace>GAZ</oboInOwl:hasOBONamespace>
        <oboInOwl:id>GAZ:00143984</oboInOwl:id>
        <rdfs:label>La Cudera</rdfs:label>
    </owl:NamedIndividual>
    


    <!-- http://purl.obolibrary.org/obo/GAZ_00143985 -->

    <owl:NamedIndividual rdf:about="http://purl.obolibrary.org/obo/GAZ_00143985">
        <obo:RO_0001025 rdf:resource="http://purl.obolibrary.org/obo/GAZ_00009676"/>
        <obo:IAO_0000115>A 5 km long glacier (2005) situated in the Bernese Alps in the canton of Valais in Switzerland.</obo:IAO_0000115>
        <oboInOwl:hasOBONamespace>GAZ</oboInOwl:hasOBONamespace>
        <oboInOwl:id>GAZ:00143985</oboInOwl:id>
        <rdfs:label>Mittelaletsch Glacier</rdfs:label>
    </owl:NamedIndividual>
    


    <!-- http://purl.obolibrary.org/obo/GAZ_00143986 -->

    <owl:NamedIndividual rdf:about="http://purl.obolibrary.org/obo/GAZ_00143986">
        <obo:RO_0001025 rdf:resource="http://purl.obolibrary.org/obo/GAZ_00008403"/>
        <obo:IAO_0000115>A 3 km long glacier (2005) situated in the Pennine Alps in the canton of Valais in Switzerland.</obo:IAO_0000115>
        <oboInOwl:hasOBONamespace>GAZ</oboInOwl:hasOBONamespace>
        <oboInOwl:id>GAZ:00143986</oboInOwl:id>
        <rdfs:label>Moming Glacier</rdfs:label>
    </owl:NamedIndividual>
    


    <!-- http://purl.obolibrary.org/obo/GAZ_00143987 -->

    <owl:NamedIndividual rdf:about="http://purl.obolibrary.org/obo/GAZ_00143987">
        <obo:RO_0001025 rdf:resource="http://purl.obolibrary.org/obo/GAZ_00009680"/>
        <obo:IAO_0000115>A 3.5 km long glacier (2005) situated in the Lepontine Alps in the canton of Graubunden in Switzerland.</obo:IAO_0000115>
        <oboInOwl:hasOBONamespace>GAZ</oboInOwl:hasOBONamespace>
        <oboInOwl:id>GAZ:00143987</oboInOwl:id>
        <rdfs:label>Paradies Glacier</rdfs:label>
    </owl:NamedIndividual>
    


    <!-- http://purl.obolibrary.org/obo/GAZ_00143988 -->

    <owl:NamedIndividual rdf:about="http://purl.obolibrary.org/obo/GAZ_00143988">
        <obo:RO_0001025 rdf:resource="http://purl.obolibrary.org/obo/GAZ_00009676"/>
        <obo:IAO_0000115>A glacier located at an elevation of 2750 m, in the canton of Bern in Switzerland. The ice field, which covers ten square km, is located below the mountain of Wildstrubel in the Bernese Alps.</obo:IAO_0000115>
        <oboInOwl:hasOBONamespace>GAZ</oboInOwl:hasOBONamespace>
        <oboInOwl:id>GAZ:00143988</oboInOwl:id>
        <rdfs:label>Plaine Morte</rdfs:label>
    </owl:NamedIndividual>
    


    <!-- http://purl.obolibrary.org/obo/GAZ_00143989 -->

    <owl:NamedIndividual rdf:about="http://purl.obolibrary.org/obo/GAZ_00143989">
        <obo:RO_0001025 rdf:resource="http://purl.obolibrary.org/obo/GAZ_00057283"/>
        <obo:IAO_0000115>A 2 km long glacier (2005) situated in the Albula Range in the canton of Graubunden in Switzerland.</obo:IAO_0000115>
        <oboInOwl:hasOBONamespace>GAZ</oboInOwl:hasOBONamespace>
        <oboInOwl:id>GAZ:00143989</oboInOwl:id>
        <rdfs:label>Porchabella Glacier</rdfs:label>
    </owl:NamedIndividual>
    


    <!-- http://purl.obolibrary.org/obo/GAZ_00143990 -->

    <owl:NamedIndividual rdf:about="http://purl.obolibrary.org/obo/GAZ_00143990">
        <obo:RO_0001025 rdf:resource="http://purl.obolibrary.org/obo/GAZ_00009676"/>
        <obo:IAO_0000115>A 5-km-long glacier (2005) situated in the Bernese Alps in the canton of Berne in Switzerland.</obo:IAO_0000115>
        <oboInOwl:hasOBONamespace>GAZ</oboInOwl:hasOBONamespace>
        <oboInOwl:id>GAZ:00143990</oboInOwl:id>
        <rdfs:label>Rosenlaui Glacier</rdfs:label>
    </owl:NamedIndividual>
    


    <!-- http://purl.obolibrary.org/obo/GAZ_00143991 -->

    <owl:NamedIndividual rdf:about="http://purl.obolibrary.org/obo/GAZ_00143991">
        <obo:RO_0001025 rdf:resource="http://purl.obolibrary.org/obo/GAZ_00008403"/>
        <obo:IAO_0000115>A 3.5 km long glacier (2005) situated in the Pennine Alps in the canton of Valais in Switzerland.</obo:IAO_0000115>
        <oboInOwl:hasOBONamespace>GAZ</oboInOwl:hasOBONamespace>
        <oboInOwl:id>GAZ:00143991</oboInOwl:id>
        <rdfs:label>Rossbode Glacier</rdfs:label>
    </owl:NamedIndividual>
    


    <!-- http://purl.obolibrary.org/obo/GAZ_00143992 -->

    <owl:NamedIndividual rdf:about="http://purl.obolibrary.org/obo/GAZ_00143992">
        <obo:RO_0001025 rdf:resource="http://purl.obolibrary.org/obo/GAZ_00008403"/>
        <obo:IAO_0000115>A 3 km long glacier (2005) situated in the Pennine Alps in the canton of Valais in Switzerland.</obo:IAO_0000115>
        <oboInOwl:hasOBONamespace>GAZ</oboInOwl:hasOBONamespace>
        <oboInOwl:id>GAZ:00143992</oboInOwl:id>
        <rdfs:label>Schwarzberg Glacier</rdfs:label>
    </owl:NamedIndividual>
    


    <!-- http://purl.obolibrary.org/obo/GAZ_00143993 -->

    <owl:NamedIndividual rdf:about="http://purl.obolibrary.org/obo/GAZ_00143993">
        <obo:RO_0001025 rdf:resource="http://purl.obolibrary.org/obo/GAZ_00057284"/>
        <obo:IAO_0000115>A 3 km long glacier (2005) situated in the Silvretta Range in the canton of Graubunden in Switzerland.</obo:IAO_0000115>
        <oboInOwl:hasOBONamespace>GAZ</oboInOwl:hasOBONamespace>
        <oboInOwl:id>GAZ:00143993</oboInOwl:id>
        <rdfs:label>Silvretta Glacier</rdfs:label>
    </owl:NamedIndividual>
    


    <!-- http://purl.obolibrary.org/obo/GAZ_00143994 -->

    <owl:NamedIndividual rdf:about="http://purl.obolibrary.org/obo/GAZ_00143994">
        <obo:RO_0001025 rdf:resource="http://purl.obolibrary.org/obo/GAZ_00056810"/>
        <obo:IAO_0000115>A 4 km long glacier (2005) situated in the Urner Alps in the canton of Berne in Switzerland.</obo:IAO_0000115>
        <oboInOwl:hasOBONamespace>GAZ</oboInOwl:hasOBONamespace>
        <oboInOwl:id>GAZ:00143994</oboInOwl:id>
        <rdfs:label>Stein Glacier</rdfs:label>
    </owl:NamedIndividual>
    


    <!-- http://purl.obolibrary.org/obo/GAZ_00143995 -->

    <owl:NamedIndividual rdf:about="http://purl.obolibrary.org/obo/GAZ_00143995">
        <obo:RO_0001025 rdf:resource="http://purl.obolibrary.org/obo/GAZ_00056810"/>
        <obo:IAO_0000115>A 2.5 km long glacier (2005) situated in the Urner Alps in the canton of Uri in Switzerland.</obo:IAO_0000115>
        <oboInOwl:hasOBONamespace>GAZ</oboInOwl:hasOBONamespace>
        <oboInOwl:id>GAZ:00143995</oboInOwl:id>
        <rdfs:label>Tiefen Glacier</rdfs:label>
    </owl:NamedIndividual>
    


    <!-- http://purl.obolibrary.org/obo/GAZ_00143996 -->

    <owl:NamedIndividual rdf:about="http://purl.obolibrary.org/obo/GAZ_00143996">
        <obo:RO_0001025 rdf:resource="http://purl.obolibrary.org/obo/GAZ_00143973"/>
        <obo:IAO_0000115>A 3.5 km long glacier (2005) situated in the Bernese Alps in the canton of Valais in Switzerland.</obo:IAO_0000115>
        <oboInOwl:hasOBONamespace>GAZ</oboInOwl:hasOBONamespace>
        <oboInOwl:id>GAZ:00143996</oboInOwl:id>
        <rdfs:label>Tsanfleuron Glacier</rdfs:label>
    </owl:NamedIndividual>
    


    <!-- http://purl.obolibrary.org/obo/GAZ_00143997 -->

    <owl:NamedIndividual rdf:about="http://purl.obolibrary.org/obo/GAZ_00143997">
        <obo:RO_0001025 rdf:resource="http://purl.obolibrary.org/obo/GAZ_00009676"/>
        <obo:IAO_0000115>A 2.5 km long glacier (2005) situated in the Bernese Alps in the canton of Valais in Switzerland.</obo:IAO_0000115>
        <oboInOwl:hasOBONamespace>GAZ</oboInOwl:hasOBONamespace>
        <oboInOwl:id>GAZ:00143997</oboInOwl:id>
        <rdfs:label>Wildstrubel Glacier</rdfs:label>
    </owl:NamedIndividual>
    


    <!-- http://purl.obolibrary.org/obo/GAZ_00143998 -->

    <owl:NamedIndividual rdf:about="http://purl.obolibrary.org/obo/GAZ_00143998">
        <obo:RO_0001025 rdf:resource="http://purl.obolibrary.org/obo/GAZ_00057284"/>
        <obo:IAO_0000115>A 2 km long glacier (2005) situated in the Silvretta Range in the canton of Graubunden in Switzerland.</obo:IAO_0000115>
        <oboInOwl:hasOBONamespace>GAZ</oboInOwl:hasOBONamespace>
        <oboInOwl:id>GAZ:00143998</oboInOwl:id>
        <rdfs:label>Verstancla Glacier</rdfs:label>
    </owl:NamedIndividual>
    


    <!-- http://purl.obolibrary.org/obo/GAZ_00143999 -->

    <owl:NamedIndividual rdf:about="http://purl.obolibrary.org/obo/GAZ_00143999">
        <obo:RO_0001025 rdf:resource="http://purl.obolibrary.org/obo/GAZ_00008403"/>
        <obo:IAO_0000115>A 3.5 km long glacier (2005) situated in the Pennine Alps in the canton of Valais in Switzerland.</obo:IAO_0000115>
        <oboInOwl:hasOBONamespace>GAZ</oboInOwl:hasOBONamespace>
        <oboInOwl:id>GAZ:00143999</oboInOwl:id>
        <rdfs:label>Valsorey Glacier</rdfs:label>
    </owl:NamedIndividual>
    


    <!-- http://purl.obolibrary.org/obo/GAZ_00144000 -->

    <owl:NamedIndividual rdf:about="http://purl.obolibrary.org/obo/GAZ_00144000">
        <obo:RO_0001025 rdf:resource="http://purl.obolibrary.org/obo/GAZ_00008403"/>
        <obo:IAO_0000115>A 5 km long glacier (2005) situated in the Pennine Alps in the canton of Valais in Switzerland.</obo:IAO_0000115>
        <oboInOwl:hasOBONamespace>GAZ</oboInOwl:hasOBONamespace>
        <oboInOwl:id>GAZ:00144000</oboInOwl:id>
        <rdfs:label>Turtmann Glacier</rdfs:label>
    </owl:NamedIndividual>
    


    <!-- http://purl.obolibrary.org/obo/GAZ_00144001 -->

    <owl:NamedIndividual rdf:about="http://purl.obolibrary.org/obo/GAZ_00144001">
        <obo:RO_0001025 rdf:resource="http://purl.obolibrary.org/obo/GAZ_00008403"/>
        <obo:IAO_0000115>A 5 km long glacier (2005) situated in the Pennine Alps in the canton of Valais in Switzerland.</obo:IAO_0000115>
        <oboInOwl:hasOBONamespace>GAZ</oboInOwl:hasOBONamespace>
        <oboInOwl:id>GAZ:00144001</oboInOwl:id>
        <rdfs:label>Moiry Glacier</rdfs:label>
    </owl:NamedIndividual>
    


    <!-- http://purl.obolibrary.org/obo/GAZ_00144002 -->

    <owl:NamedIndividual rdf:about="http://purl.obolibrary.org/obo/GAZ_00144002">
        <obo:RO_0001025 rdf:resource="http://purl.obolibrary.org/obo/GAZ_00009676"/>
        <obo:IAO_0000115>A 4 km long glacier (2005) situated in the Bernese Alps in the canton of Valais in Switzerland.</obo:IAO_0000115>
        <oboInOwl:hasOBONamespace>GAZ</oboInOwl:hasOBONamespace>
        <oboInOwl:id>GAZ:00144002</oboInOwl:id>
        <rdfs:label>Tsijiore Nouve Glacier</rdfs:label>
    </owl:NamedIndividual>
    


    <!-- http://purl.obolibrary.org/obo/GAZ_00144003 -->

    <owl:NamedIndividual rdf:about="http://purl.obolibrary.org/obo/GAZ_00144003">
        <obo:RO_0001025 rdf:resource="http://purl.obolibrary.org/obo/GAZ_00009680"/>
        <obo:IAO_0000115>A 5 km long glacier (2005) situated in the Lepontine Alps in the canton of Valais in Switzerland.</obo:IAO_0000115>
        <oboInOwl:hasOBONamespace>GAZ</oboInOwl:hasOBONamespace>
        <oboInOwl:id>GAZ:00144003</oboInOwl:id>
        <rdfs:label>Gries Glacier</rdfs:label>
    </owl:NamedIndividual>
    


    <!-- http://purl.obolibrary.org/obo/GAZ_00144004 -->

    <owl:NamedIndividual rdf:about="http://purl.obolibrary.org/obo/GAZ_00144004">
        <obo:RO_0001025 rdf:resource="http://purl.obolibrary.org/obo/GAZ_00056784"/>
        <obo:IAO_0000115>The longest glacier in Austria and in the Eastern Alps. It lies within the Hohe Tauern mountain range in Carinthia, directly beneath Austria&apos;s highest mountain, the Grossglockner.</obo:IAO_0000115>
        <oboInOwl:hasOBONamespace>GAZ</oboInOwl:hasOBONamespace>
        <oboInOwl:id>GAZ:00144004</oboInOwl:id>
        <rdfs:label>Pasterze Glacier</rdfs:label>
    </owl:NamedIndividual>
    


    <!-- http://purl.obolibrary.org/obo/GAZ_00144005 -->

    <owl:NamedIndividual rdf:about="http://purl.obolibrary.org/obo/GAZ_00144005">
        <obo:RO_0001025 rdf:resource="http://purl.obolibrary.org/obo/GAZ_00056784"/>
        <obo:RO_0001025 rdf:resource="http://purl.obolibrary.org/obo/GAZ_00179296"/>
        <obo:IAO_0000115>A glacier.</obo:IAO_0000115>
        <oboInOwl:hasOBONamespace>GAZ</oboInOwl:hasOBONamespace>
        <oboInOwl:id>GAZ:00144005</oboInOwl:id>
        <rdfs:label>Kitzsteinhorn Glacier</rdfs:label>
    </owl:NamedIndividual>
    


    <!-- http://purl.obolibrary.org/obo/GAZ_00144361 -->

    <owl:NamedIndividual rdf:about="http://purl.obolibrary.org/obo/GAZ_00144361">
        <obo:RO_0001025 rdf:resource="http://purl.obolibrary.org/obo/GAZ_00179752"/>
        <obo:IAO_0000115>The estuary of the Scheldt river.</obo:IAO_0000115>
        <oboInOwl:hasOBONamespace>GAZ</oboInOwl:hasOBONamespace>
        <oboInOwl:id>GAZ:00144361</oboInOwl:id>
        <rdfs:label>Westerschelde</rdfs:label>
    </owl:NamedIndividual>
    


    <!-- http://purl.obolibrary.org/obo/GAZ_00144362 -->

    <owl:NamedIndividual rdf:about="http://purl.obolibrary.org/obo/GAZ_00144362">
        <obo:RO_0001025 rdf:resource="http://purl.obolibrary.org/obo/GAZ_00090210"/>
        <obo:IAO_0000115>A former island, now peninsula, crossed by the Canal through Zuid-Beveland on the west and the Scheldt-Rhine Canal on the east.</obo:IAO_0000115>
        <oboInOwl:hasOBONamespace>GAZ</oboInOwl:hasOBONamespace>
        <oboInOwl:id>GAZ:00144362</oboInOwl:id>
        <rdfs:label>Zuid-Beveland</rdfs:label>
    </owl:NamedIndividual>
    


    <!-- http://purl.obolibrary.org/obo/GAZ_00144364 -->

    <owl:NamedIndividual rdf:about="http://purl.obolibrary.org/obo/GAZ_00144364">
        <obo:RO_0001025 rdf:resource="http://purl.obolibrary.org/obo/GAZ_00144362"/>
        <obo:IAO_0000115>A canal in the Netherlands that is the western of the two canals crossing Zuid-Beveland. It connects the Westerschelde and the Oosterschelde.</obo:IAO_0000115>
        <oboInOwl:hasOBONamespace>GAZ</oboInOwl:hasOBONamespace>
        <oboInOwl:id>GAZ:00144364</oboInOwl:id>
        <rdfs:label>Kanaal door Zuid-Beveland</rdfs:label>
    </owl:NamedIndividual>
    


    <!-- http://purl.obolibrary.org/obo/GAZ_00144365 -->

    <owl:NamedIndividual rdf:about="http://purl.obolibrary.org/obo/GAZ_00144365">
        <obo:RO_0001025 rdf:resource="http://purl.obolibrary.org/obo/GAZ_00325162"/>
        <obo:IAO_0000115>A former tidal branch of river Scheldt that has been channelised to form the northern stretch of the Scheldt-Rhine Canal. It flows from the Markiezaatsmeer lake (formerly part of the Oosterschelde) near Bergen op Zoom past the town and eponymous island of Tholen towards the former island of Sint-Philipsland, where it used to end in the Krabbenkreek estuary. The passage to the estuary has been closed off, however, and an additional stretch of canal was dug to connect the Eendracht to the Krammer lake, itself a former estuary closed off from the sea during the Delta Works.</obo:IAO_0000115>
        <oboInOwl:hasOBONamespace>GAZ</oboInOwl:hasOBONamespace>
        <oboInOwl:id>GAZ:00144365</oboInOwl:id>
        <rdfs:label>Eendracht</rdfs:label>
    </owl:NamedIndividual>
    


    <!-- http://purl.obolibrary.org/obo/GAZ_00144366 -->

    <owl:NamedIndividual rdf:about="http://purl.obolibrary.org/obo/GAZ_00144366">
        <obo:RO_0001025 rdf:resource="http://purl.obolibrary.org/obo/GAZ_00021226"/>
        <obo:IAO_0000115>A former strait, now a bay, that separates Tholen Island and Sint Philipsland Island.</obo:IAO_0000115>
        <oboInOwl:hasOBONamespace>GAZ</oboInOwl:hasOBONamespace>
        <oboInOwl:id>GAZ:00144366</oboInOwl:id>
        <rdfs:label>Krabbenkreek</rdfs:label>
    </owl:NamedIndividual>
    


    <!-- http://purl.obolibrary.org/obo/GAZ_00144367 -->

    <owl:NamedIndividual rdf:about="http://purl.obolibrary.org/obo/GAZ_00144367">
        <obo:RO_0001025 rdf:resource="http://purl.obolibrary.org/obo/GAZ_00090210"/>
        <obo:IAO_0000115>A strait.</obo:IAO_0000115>
        <oboInOwl:hasOBONamespace>GAZ</oboInOwl:hasOBONamespace>
        <oboInOwl:id>GAZ:00144367</oboInOwl:id>
        <rdfs:label>Krammer</rdfs:label>
    </owl:NamedIndividual>
    


    <!-- http://purl.obolibrary.org/obo/GAZ_00144368 -->

    <owl:NamedIndividual rdf:about="http://purl.obolibrary.org/obo/GAZ_00144368">
        <obo:RO_0001025 rdf:resource="http://purl.obolibrary.org/obo/GAZ_00090210"/>
        <obo:IAO_0000115>A strait.</obo:IAO_0000115>
        <oboInOwl:hasOBONamespace>GAZ</oboInOwl:hasOBONamespace>
        <oboInOwl:id>GAZ:00144368</oboInOwl:id>
        <rdfs:label>Keeten-Mastgat</rdfs:label>
    </owl:NamedIndividual>
    


    <!-- http://purl.obolibrary.org/obo/GAZ_00144369 -->

    <owl:NamedIndividual rdf:about="http://purl.obolibrary.org/obo/GAZ_00144369">
        <obo:RO_0001025 rdf:resource="http://purl.obolibrary.org/obo/GAZ_00144361"/>
        <obo:IAO_0000115>A former large tidal inlet in the middle of the Dutch region of Zeeuws-Vlaanderen, on the south bank of the Westerschelde west of Terneuzen. Closed from the estuary after 1960.</obo:IAO_0000115>
        <oboInOwl:hasOBONamespace>GAZ</oboInOwl:hasOBONamespace>
        <oboInOwl:id>GAZ:00144369</oboInOwl:id>
        <rdfs:label>Braakman</rdfs:label>
    </owl:NamedIndividual>
    


    <!-- http://purl.obolibrary.org/obo/GAZ_00144371 -->

    <owl:NamedIndividual rdf:about="http://purl.obolibrary.org/obo/GAZ_00144371">
        <obo:RO_0001025 rdf:resource="http://purl.obolibrary.org/obo/GAZ_00144361"/>
        <obo:IAO_0000115>A former island in the province of Zeeland in the Netherlands at the mouth of the Scheldt estuary. It lies between the Oosterschelde in the north and the Westerschelde in the south and is roughly the shape of a rhombus. The two sides on the side of the North Sea consist of dunes; the rest of its coastline is made up of dykes. Middelburg lies at its centre; this city is the provincial capital and Vlissingen 9 km to the south is the main harbour. The third municipality is Veere. Originally, Walcheren was an island, but polders and a dam across the Sloe strait have connected it to the (former) island of Zuid-Beveland, which in turn has been connected to the North Brabant mainland.</obo:IAO_0000115>
        <oboInOwl:hasOBONamespace>GAZ</oboInOwl:hasOBONamespace>
        <oboInOwl:id>GAZ:00144371</oboInOwl:id>
        <rdfs:label>Walcheren</rdfs:label>
    </owl:NamedIndividual>
    


    <!-- http://purl.obolibrary.org/obo/GAZ_00144373 -->

    <owl:NamedIndividual rdf:about="http://purl.obolibrary.org/obo/GAZ_00144373">
        <obo:RO_0001025 rdf:resource="http://purl.obolibrary.org/obo/GAZ_00090210"/>
        <obo:IAO_0000115>A former island now enclosed by the Oosterschelde estuary to the north, and the former straits, now combined lake, of Veerse Meer and Zandkreek to the south. As part of the Delta Works, dams have connected Noord-Beveland to Walcheren and Zuid-Beveland.</obo:IAO_0000115>
        <oboInOwl:hasOBONamespace>GAZ</oboInOwl:hasOBONamespace>
        <oboInOwl:id>GAZ:00144373</oboInOwl:id>
        <rdfs:label>Noord-Beveland</rdfs:label>
    </owl:NamedIndividual>
    


    <!-- http://purl.obolibrary.org/obo/GAZ_00144376 -->

    <owl:NamedIndividual rdf:about="http://purl.obolibrary.org/obo/GAZ_00144376">
        <obo:RO_0001025 rdf:resource="http://purl.obolibrary.org/obo/GAZ_00008262"/>
        <obo:IAO_0000115>A river delta in The Netherlands formed by the confluence of the Rhine, the Meuse and the Scheldt rivers. The result is a multitude of islands, branches and branch names that may at first sight look bewildering, especially as a waterway that appears to be one continuous stream may change names as many as seven times (e.g. Rhine &gt; Bijlands Kanaal &gt; Pannerdens Kanaal &gt; Nederrijn &gt; Lek &gt; Nieuwe Maas &gt; Het Scheur &gt; Nieuwe Waterweg (&gt; North Sea)).</obo:IAO_0000115>
        <oboInOwl:hasOBONamespace>GAZ</oboInOwl:hasOBONamespace>
        <oboInOwl:id>GAZ:00144376</oboInOwl:id>
        <rdfs:label>Rijn-Maas-Scheldedelta</rdfs:label>
    </owl:NamedIndividual>
    


    <!-- http://purl.obolibrary.org/obo/GAZ_00144377 -->

    <owl:NamedIndividual rdf:about="http://purl.obolibrary.org/obo/GAZ_00144377">
        <rdf:type rdf:resource="http://purl.obolibrary.org/obo/ENVO_00000029"/>
        <obo:RO_0001025 rdf:resource="http://purl.obolibrary.org/obo/GAZ_00144376"/>
        <obo:IAO_0000115>A branch of the Rhine-Meuse delta in South Holland, the Netherlands, that flows west from the confluence of the Oude Maas and Nieuwe Maas branches past the towns of Rozenburg and Maassluis. It continues as the Nieuwe Waterweg (New Waterway) to the North Sea. Originally, Het Scheur was the northern branch of the river around Rozenburg island and curved south a few km past Maassluis to join the Nieuwe Maas again in the Maasmond (&quot;Mouth of Meuse&quot;) estuary near Den Briel. When the Nieuwe Waterweg was completed in 1872, Het Scheur was dammed off and connected to the east end of the Nieuwe Waterweg to form the new channelized main mouth of the Rhine-Meuse delta.</obo:IAO_0000115>
        <oboInOwl:hasOBONamespace>GAZ</oboInOwl:hasOBONamespace>
        <oboInOwl:id>GAZ:00144377</oboInOwl:id>
        <rdfs:label>Het Scheur</rdfs:label>
    </owl:NamedIndividual>
    


    <!-- http://purl.obolibrary.org/obo/GAZ_00144378 -->

    <owl:NamedIndividual rdf:about="http://purl.obolibrary.org/obo/GAZ_00144378">
        <rdf:type rdf:resource="http://purl.obolibrary.org/obo/ENVO_00000029"/>
        <obo:RO_0001025 rdf:resource="http://purl.obolibrary.org/obo/GAZ_00144376"/>
        <obo:IAO_0000115>A branch in the Rhine-Meuse delta in the Dutch province of South Holland. It begins at the city of Dordrecht where the Beneden Merwede river splits into the Noord River and the Oude Maas.</obo:IAO_0000115>
        <oboInOwl:hasOBONamespace>GAZ</oboInOwl:hasOBONamespace>
        <oboInOwl:id>GAZ:00144378</oboInOwl:id>
        <rdfs:label>Oude Maas</rdfs:label>
    </owl:NamedIndividual>
    


    <!-- http://purl.obolibrary.org/obo/GAZ_00144379 -->

    <owl:NamedIndividual rdf:about="http://purl.obolibrary.org/obo/GAZ_00144379">
        <obo:RO_0001025 rdf:resource="http://purl.obolibrary.org/obo/GAZ_00144376"/>
        <obo:IAO_0000115>The main distributary branch of river Rhine flowing to the central Netherlands for about 80 km before joining the Meuse near Woudrichem to form the Boven Merwede. It is a major river which serves as the main waterway connecting the Rotterdam harbor and Germany.</obo:IAO_0000115>
        <oboInOwl:hasOBONamespace>GAZ</oboInOwl:hasOBONamespace>
        <oboInOwl:id>GAZ:00144379</oboInOwl:id>
        <rdfs:label>Waal</rdfs:label>
    </owl:NamedIndividual>
    


    <!-- http://purl.obolibrary.org/obo/GAZ_00144380 -->

    <owl:NamedIndividual rdf:about="http://purl.obolibrary.org/obo/GAZ_00144380">
        <obo:RO_0001025 rdf:resource="http://purl.obolibrary.org/obo/GAZ_00043990"/>
        <obo:IAO_0000115>A former river island, the western branch of river Waal separating it from IJsselmonde. However, as the Waal stretch has been closed off at both ends, the Waard is now generally considered to be part of IJsselmonde.</obo:IAO_0000115>
        <oboInOwl:hasOBONamespace>GAZ</oboInOwl:hasOBONamespace>
        <oboInOwl:id>GAZ:00144380</oboInOwl:id>
        <rdfs:label>Zwijndrechtse Waard</rdfs:label>
    </owl:NamedIndividual>
    


    <!-- http://purl.obolibrary.org/obo/GAZ_00144381 -->

    <owl:NamedIndividual rdf:about="http://purl.obolibrary.org/obo/GAZ_00144381">
        <obo:RO_0001025 rdf:resource="http://purl.obolibrary.org/obo/GAZ_00144376"/>
        <obo:IAO_0000115>An island between the Oude Maas, Dordtsche Kil, Hollands Diep, Haringvliet and Spui rivers in the province of Zuid Holland in the Netherlands.</obo:IAO_0000115>
        <oboInOwl:hasOBONamespace>GAZ</oboInOwl:hasOBONamespace>
        <oboInOwl:id>GAZ:00144381</oboInOwl:id>
        <rdfs:label>Hoeksche Waard</rdfs:label>
    </owl:NamedIndividual>
    


    <!-- http://purl.obolibrary.org/obo/GAZ_00144382 -->

    <owl:NamedIndividual rdf:about="http://purl.obolibrary.org/obo/GAZ_00144382">
        <obo:RO_0001025 rdf:resource="http://purl.obolibrary.org/obo/GAZ_00144376"/>
        <obo:IAO_0000115>A small tidal river in South Holland in the Netherlands, separating the islands of Voorne-Putten and Hoekse Waard. Historically, it forked off the Oude Maas river at the town of Oud-Beijerland to end in the Haringvliet estuary, but as a (planned) result from the Delta Works, its flow has been reversed.</obo:IAO_0000115>
        <oboInOwl:hasOBONamespace>GAZ</oboInOwl:hasOBONamespace>
        <oboInOwl:id>GAZ:00144382</oboInOwl:id>
        <rdfs:label>Spui</rdfs:label>
    </owl:NamedIndividual>
    


    <!-- http://purl.obolibrary.org/obo/GAZ_00144383 -->

    <owl:NamedIndividual rdf:about="http://purl.obolibrary.org/obo/GAZ_00144383">
        <obo:RO_0001025 rdf:resource="http://purl.obolibrary.org/obo/GAZ_00144376"/>
        <obo:IAO_0000115>A large inlet of the North Sea, in the province of South Holland in the Netherlands. It is an important estuary of the Rhine-Meuse delta. Near Numansdorp, the Hollands Diep splits into the Haringvliet and the Volkerak estuaries. It is closed off near Goedereede from the North Sea by the Haringvliet sluices, which provide a road connection between the island of Voorne to the north and the island of Goeree-Overflakkee to the south. The sluices were built as part of the Delta Works sea barrier protection works, and allow for a brackish ecological environment.</obo:IAO_0000115>
        <oboInOwl:hasOBONamespace>GAZ</oboInOwl:hasOBONamespace>
        <oboInOwl:id>GAZ:00144383</oboInOwl:id>
        <rdfs:label>Haringvliet</rdfs:label>
    </owl:NamedIndividual>
    


    <!-- http://purl.obolibrary.org/obo/GAZ_00144384 -->

    <owl:NamedIndividual rdf:about="http://purl.obolibrary.org/obo/GAZ_00144384">
        <obo:RO_0001025 rdf:resource="http://purl.obolibrary.org/obo/GAZ_00144376"/>
        <obo:IAO_0000115>A wide river in the Netherlands and an estuary of the Rhine and Meuse river. Through the Scheldt-Rhine Canal it connects to the Scheldt river and Antwerp.</obo:IAO_0000115>
        <oboInOwl:hasOBONamespace>GAZ</oboInOwl:hasOBONamespace>
        <oboInOwl:id>GAZ:00144384</oboInOwl:id>
        <rdfs:label>Hollands Diep</rdfs:label>
    </owl:NamedIndividual>
    


    <!-- http://purl.obolibrary.org/obo/GAZ_00144386 -->

    <owl:NamedIndividual rdf:about="http://purl.obolibrary.org/obo/GAZ_00144386">
        <obo:RO_0001025 rdf:resource="http://purl.obolibrary.org/obo/GAZ_00144376"/>
        <obo:IAO_0000115>A canal that was constructed in 1904 to be a branch of the Meuse River in the Dutch province of Noord-Brabant. The river Meuse splits near Heusden into the Afgedamde Maas and the Berge Maas. The Afgedamde Maas flows north until its confluence with the river Waal (Rhine), while the Berge Maas flows west as the main distributary branch. Historically, a natural Meuse branch flowed from Heusden to the Amer and Hollands Diep estuary; this branch silted up and now forms the stream called Oude Maasje. The Bergse Maas was constructed in its basin to take over its functions.</obo:IAO_0000115>
        <oboInOwl:hasOBONamespace>GAZ</oboInOwl:hasOBONamespace>
        <oboInOwl:id>GAZ:00144386</oboInOwl:id>
        <rdfs:label>Bergse Maas</rdfs:label>
    </owl:NamedIndividual>
    


    <!-- http://purl.obolibrary.org/obo/GAZ_00144387 -->

    <owl:NamedIndividual rdf:about="http://purl.obolibrary.org/obo/GAZ_00144387">
        <obo:RO_0001025 rdf:resource="http://purl.obolibrary.org/obo/GAZ_00144376"/>
        <obo:IAO_0000115>A N branch of the Maas River after the split near Heusden.</obo:IAO_0000115>
        <oboInOwl:hasOBONamespace>GAZ</oboInOwl:hasOBONamespace>
        <oboInOwl:id>GAZ:00144387</oboInOwl:id>
        <rdfs:label>Afgedamde Maas</rdfs:label>
    </owl:NamedIndividual>
    


    <!-- http://purl.obolibrary.org/obo/GAZ_00144388 -->

    <owl:NamedIndividual rdf:about="http://purl.obolibrary.org/obo/GAZ_00144388">
        <obo:RO_0001025 rdf:resource="http://purl.obolibrary.org/obo/GAZ_00144419"/>
        <obo:IAO_0000115>A stretch of river in the Netherlands. The Afgedamde Maas river joins the Waal at Woudrichem to form the Boven Merwede, which at Hardinxveld-Giessendam splits into the Beneden Merwede river on the right and the Nieuwe Merwede river on the left. Its length is 8.8 km. The Merwede is part of the main shipping route between Rotterdam and Germany.</obo:IAO_0000115>
        <oboInOwl:hasOBONamespace>GAZ</oboInOwl:hasOBONamespace>
        <oboInOwl:id>GAZ:00144388</oboInOwl:id>
        <rdfs:label>Boven Merwede</rdfs:label>
    </owl:NamedIndividual>
    


    <!-- http://purl.obolibrary.org/obo/GAZ_00144389 -->

    <owl:NamedIndividual rdf:about="http://purl.obolibrary.org/obo/GAZ_00144389">
        <obo:RO_0001025 rdf:resource="http://purl.obolibrary.org/obo/GAZ_00144419"/>
        <obo:IAO_0000115>A canal that was constructed in 1870 to form a branch in the Rhine-Meuse delta. It was dug along the general trajectories of a number of minor Biesbosch creeks to reduce the risk of flooding by diverting the water away from the Beneden Merwede, and to facilitate navigation and regulate river traffic in the increasingly silted-up delta.</obo:IAO_0000115>
        <oboInOwl:hasOBONamespace>GAZ</oboInOwl:hasOBONamespace>
        <oboInOwl:id>GAZ:00144389</oboInOwl:id>
        <rdfs:label>Nieuwe Merwede</rdfs:label>
    </owl:NamedIndividual>
    


    <!-- http://purl.obolibrary.org/obo/GAZ_00144390 -->

    <owl:NamedIndividual rdf:about="http://purl.obolibrary.org/obo/GAZ_00144390">
        <obo:RO_0001025 rdf:resource="http://purl.obolibrary.org/obo/GAZ_00144419"/>
        <obo:IAO_0000115>A stretch of river in the Netherlands, the continuation of the Boven Merwede after the branching-off of the Nieuwe Merwede ship canal. It flows from Hardinxveld-Giessendam to Dordrecht, where it splits into the Noord and Oude Maas rivers. Its length is 14.9 km. The Merwede is part of the main shipping route between Rotterdam and Germany.</obo:IAO_0000115>
        <oboInOwl:hasOBONamespace>GAZ</oboInOwl:hasOBONamespace>
        <oboInOwl:id>GAZ:00144390</oboInOwl:id>
        <rdfs:label>Beneden Merwede</rdfs:label>
    </owl:NamedIndividual>
    


    <!-- http://purl.obolibrary.org/obo/GAZ_00144391 -->

    <owl:NamedIndividual rdf:about="http://purl.obolibrary.org/obo/GAZ_00144391">
        <obo:RO_0001025 rdf:resource="http://purl.obolibrary.org/obo/GAZ_00144376"/>
        <obo:IAO_0000115>A short river in South Holland in the Netherlands. The river is tidal and forms the connection between the Oude Maas river and the Hollands Diep. The river is for most part artificial in origin, since it has been a relatively small tidal creek until the 19th century.</obo:IAO_0000115>
        <oboInOwl:hasOBONamespace>GAZ</oboInOwl:hasOBONamespace>
        <oboInOwl:id>GAZ:00144391</oboInOwl:id>
        <rdfs:label>Dordtsche Kil</rdfs:label>
    </owl:NamedIndividual>
    


    <!-- http://purl.obolibrary.org/obo/GAZ_00144392 -->

    <owl:NamedIndividual rdf:about="http://purl.obolibrary.org/obo/GAZ_00144392">
        <obo:RO_0001025 rdf:resource="http://purl.obolibrary.org/obo/GAZ_00144376"/>
        <obo:IAO_0000115>A river branch of the Rhine-Meuse delta in the Netherlands. It runs from the confluence of the rivers Noord and Lek, and flows west through Rotterdam. It ends west of the city where it meets the Oude Maas, near Vlaardingen, to form Het Scheur. The total length is approximately 24 km.</obo:IAO_0000115>
        <oboInOwl:hasOBONamespace>GAZ</oboInOwl:hasOBONamespace>
        <oboInOwl:id>GAZ:00144392</oboInOwl:id>
        <rdfs:label>Nieuwe Maas</rdfs:label>
    </owl:NamedIndividual>
    


    <!-- http://purl.obolibrary.org/obo/GAZ_00144393 -->

    <owl:NamedIndividual rdf:about="http://purl.obolibrary.org/obo/GAZ_00144393">
        <obo:RO_0001025 rdf:resource="http://purl.obolibrary.org/obo/GAZ_00144376"/>
        <obo:IAO_0000115>A ship canal in the Netherlands from Het Scheur (a branch of the Rhine-Meuse-Scheldt delta) west of the town of Maassluis to the North Sea at Hook of Holland. It is the artificial mouth of the river Rhine. The Nieuwe Waterweg, which opened in 1872 and has a length of approximately 10 km.</obo:IAO_0000115>
        <oboInOwl:hasOBONamespace>GAZ</oboInOwl:hasOBONamespace>
        <oboInOwl:id>GAZ:00144393</oboInOwl:id>
        <rdfs:label>Nieuwe Waterweg</rdfs:label>
    </owl:NamedIndividual>
    


    <!-- http://purl.obolibrary.org/obo/GAZ_00144394 -->

    <owl:NamedIndividual rdf:about="http://purl.obolibrary.org/obo/GAZ_00144394">
        <obo:RO_0001025 rdf:resource="http://purl.obolibrary.org/obo/GAZ_00144392"/>
        <obo:IAO_0000115>Formerly the name of a stretch of the Nieuwe Maas river, part of the Rhine-Meuse delta near the Dutch cities of Vlaardingen and Spijkenisse in the province of Zuid-Holland. Specifically, it was the name of the strait that separated the island of Rozenburg from the sand bar of Welplaat. The strait itself was merely the continuation of the Nieuwe Maas, and the stretch of the river south of Rozenburg continued to be called Nieuwe Maas until the confluence with het Scheur formed the Brielse Maas estuary.</obo:IAO_0000115>
        <oboInOwl:hasOBONamespace>GAZ</oboInOwl:hasOBONamespace>
        <oboInOwl:id>GAZ:00144394</oboInOwl:id>
        <rdfs:label>Botlek</rdfs:label>
    </owl:NamedIndividual>
    


    <!-- http://purl.obolibrary.org/obo/GAZ_00144395 -->

    <owl:NamedIndividual rdf:about="http://purl.obolibrary.org/obo/GAZ_00144395">
        <obo:RO_0001025 rdf:resource="http://purl.obolibrary.org/obo/GAZ_00144396"/>
        <obo:IAO_0000115>The estuary of the Amer River.</obo:IAO_0000115>
        <oboInOwl:hasOBONamespace>GAZ</oboInOwl:hasOBONamespace>
        <oboInOwl:id>GAZ:00144395</oboInOwl:id>
        <rdfs:label>Amer Estuary</rdfs:label>
    </owl:NamedIndividual>
    


    <!-- http://purl.obolibrary.org/obo/GAZ_00144396 -->

    <owl:NamedIndividual rdf:about="http://purl.obolibrary.org/obo/GAZ_00144396">
        <obo:RO_0001025 rdf:resource="http://purl.obolibrary.org/obo/GAZ_00144376"/>
        <obo:IAO_0000115>A river in the Dutch province of Noord-Brabant. It is a continuation of the Bergse Maas river from the river Donge near Raamsdonksveer to the point where it joins the river Nieuwe Merwede to form the Hollands Diep estuary, and has a total length of approximately 20 km. The Amer is a major navigation route. It forms the south boundary of the Biesbosch National Park.</obo:IAO_0000115>
        <oboInOwl:hasOBONamespace>GAZ</oboInOwl:hasOBONamespace>
        <oboInOwl:id>GAZ:00144396</oboInOwl:id>
        <rdfs:label>Amer</rdfs:label>
    </owl:NamedIndividual>
    


    <!-- http://purl.obolibrary.org/obo/GAZ_00144397 -->

    <owl:NamedIndividual rdf:about="http://purl.obolibrary.org/obo/GAZ_00144397">
        <obo:RO_0001025 rdf:resource="http://purl.obolibrary.org/obo/GAZ_00144376"/>
        <obo:IAO_0000115>A former river island. When the Pannerdens Kanaal was dug between 1701 and 1709, the easternmost tip of the Betuwe (including the towns of Pannerden and Lobith) was cut off from the rest of the region. The Betuwe is situated between the Waal and Rhine/Lek rivers, surrounding the Linge stream, and is famous for its fruit production. The largest and most important city in the area is Tiel.</obo:IAO_0000115>
        <oboInOwl:hasOBONamespace>GAZ</oboInOwl:hasOBONamespace>
        <oboInOwl:id>GAZ:00144397</oboInOwl:id>
        <rdfs:label>Betuwe</rdfs:label>
    </owl:NamedIndividual>
    


    <!-- http://purl.obolibrary.org/obo/GAZ_00144398 -->

    <owl:NamedIndividual rdf:about="http://purl.obolibrary.org/obo/GAZ_00144398">
        <obo:RO_0001025 rdf:resource="http://purl.obolibrary.org/obo/GAZ_00144376"/>
        <obo:IAO_0000115>A canal in the Dutch province of Gelderland, near the Dutch-German border. It is currently by far the most important river-stretch of the Rhine when that major river enters the Netherlands. Constructed 1773-1776.</obo:IAO_0000115>
        <oboInOwl:hasOBONamespace>GAZ</oboInOwl:hasOBONamespace>
        <oboInOwl:id>GAZ:00144398</oboInOwl:id>
        <rdfs:label>Bijlands Kanaal</rdfs:label>
    </owl:NamedIndividual>
    


    <!-- http://purl.obolibrary.org/obo/GAZ_00144399 -->

    <owl:NamedIndividual rdf:about="http://purl.obolibrary.org/obo/GAZ_00144399">
        <obo:RO_0001025 rdf:resource="http://purl.obolibrary.org/obo/GAZ_00144376"/>
        <obo:IAO_0000115>A long former bend in river Rhine in the Dutch province of Gelderland. In summer the bend became too shallow to be navigable, and so between 1701 and 1709 was cut off from the main waterway near the town of Lobith and replaced by the Pannerdens Kanaal. The Oude Rijn, which forms the border between the Dutch town of Lobith and the German town of Elten, was still used to relieve overflow of the Rhine in times of flooding until the middle of the twentieth century.</obo:IAO_0000115>
        <oboInOwl:hasOBONamespace>GAZ</oboInOwl:hasOBONamespace>
        <oboInOwl:id>GAZ:00144399</oboInOwl:id>
        <rdfs:label>Oude Rijn [Gelderland]</rdfs:label>
    </owl:NamedIndividual>
    


    <!-- http://purl.obolibrary.org/obo/GAZ_00144400 -->

    <owl:NamedIndividual rdf:about="http://purl.obolibrary.org/obo/GAZ_00144400">
        <rdf:type rdf:resource="http://purl.obolibrary.org/obo/ENVO_00000029"/>
        <obo:RO_0001025 rdf:resource="http://purl.obolibrary.org/obo/GAZ_00144376"/>
        <obo:IAO_0000115>A branch of the Rhine delta in the Dutch provinces of Utrecht and South Holland. Its present-day length is 52 km.</obo:IAO_0000115>
        <oboInOwl:hasOBONamespace>GAZ</oboInOwl:hasOBONamespace>
        <oboInOwl:id>GAZ:00144400</oboInOwl:id>
        <rdfs:label>Oude Rijn [South Holland]</rdfs:label>
    </owl:NamedIndividual>
    


    <!-- http://purl.obolibrary.org/obo/GAZ_00144401 -->

    <owl:NamedIndividual rdf:about="http://purl.obolibrary.org/obo/GAZ_00144401">
        <obo:RO_0001025 rdf:resource="http://purl.obolibrary.org/obo/GAZ_00325310"/>
        <obo:IAO_0000115>The eastern and largest part of the Biesbosch, which is separated from the rest of the Biesbosch by the Nieuwe Merwede river (which serves as the borderline between the provinces of South Holland and North Brabant). The Brabantse Biesbosch can be divided in three parts, from which only the so called Zuidwaard belongs to the National Park.</obo:IAO_0000115>
        <oboInOwl:hasOBONamespace>GAZ</oboInOwl:hasOBONamespace>
        <oboInOwl:id>GAZ:00144401</oboInOwl:id>
        <rdfs:label>Brabantse Biesbosch, Zuidwaard</rdfs:label>
    </owl:NamedIndividual>
    


    <!-- http://purl.obolibrary.org/obo/GAZ_00144402 -->

    <owl:NamedIndividual rdf:about="http://purl.obolibrary.org/obo/GAZ_00144402">
        <obo:RO_0001025 rdf:resource="http://purl.obolibrary.org/obo/GAZ_00090211"/>
        <obo:IAO_0000115>The part of the Biesbosch that borders the city of Dordrecht. It is located between the Sliedrechtse Biesbosch and the Hollandse Biesbosch.</obo:IAO_0000115>
        <oboInOwl:hasOBONamespace>GAZ</oboInOwl:hasOBONamespace>
        <oboInOwl:id>GAZ:00144402</oboInOwl:id>
        <rdfs:label>Dordtse Biesbosch</rdfs:label>
    </owl:NamedIndividual>
    


    <!-- http://purl.obolibrary.org/obo/GAZ_00144403 -->

    <owl:NamedIndividual rdf:about="http://purl.obolibrary.org/obo/GAZ_00144403">
        <obo:RO_0001025 rdf:resource="http://purl.obolibrary.org/obo/GAZ_00090211"/>
        <obo:IAO_0000115>The westernmost part of the Biesbosch and the largest remnant of the (once much larger) South Hollandic part of the Biesbosch.</obo:IAO_0000115>
        <oboInOwl:hasOBONamespace>GAZ</oboInOwl:hasOBONamespace>
        <oboInOwl:id>GAZ:00144403</oboInOwl:id>
        <rdfs:label>Hollandse Biesbosch</rdfs:label>
    </owl:NamedIndividual>
    


    <!-- http://purl.obolibrary.org/obo/GAZ_00144404 -->

    <owl:NamedIndividual rdf:about="http://purl.obolibrary.org/obo/GAZ_00144404">
        <obo:RO_0001025 rdf:resource="http://purl.obolibrary.org/obo/GAZ_00090211"/>
        <obo:IAO_0000115>The most northern part of the Biesbosch. This is the part of the Biesbosch with the most significant tidal influence.</obo:IAO_0000115>
        <oboInOwl:hasOBONamespace>GAZ</oboInOwl:hasOBONamespace>
        <oboInOwl:id>GAZ:00144404</oboInOwl:id>
        <rdfs:label>Sliedrechtse Biesbosch</rdfs:label>
    </owl:NamedIndividual>
    


    <!-- http://purl.obolibrary.org/obo/GAZ_00144405 -->

    <owl:NamedIndividual rdf:about="http://purl.obolibrary.org/obo/GAZ_00144405">
        <obo:RO_0001025 rdf:resource="http://purl.obolibrary.org/obo/GAZ_00325310"/>
        <obo:IAO_0000115>The most central part of the Biesbosch.</obo:IAO_0000115>
        <oboInOwl:hasOBONamespace>GAZ</oboInOwl:hasOBONamespace>
        <oboInOwl:id>GAZ:00144405</oboInOwl:id>
        <rdfs:label>Brabantse Biesbosch, Noordwaard</rdfs:label>
    </owl:NamedIndividual>
    


    <!-- http://purl.obolibrary.org/obo/GAZ_00144406 -->

    <owl:NamedIndividual rdf:about="http://purl.obolibrary.org/obo/GAZ_00144406">
        <obo:RO_0001025 rdf:resource="http://purl.obolibrary.org/obo/GAZ_00325310"/>
        <obo:IAO_0000115>The easternmost and oldest part of the Biesbosch.</obo:IAO_0000115>
        <oboInOwl:hasOBONamespace>GAZ</oboInOwl:hasOBONamespace>
        <oboInOwl:id>GAZ:00144406</oboInOwl:id>
        <rdfs:label>Brabantse Biesbosch, Oostwaard</rdfs:label>
    </owl:NamedIndividual>
    


    <!-- http://purl.obolibrary.org/obo/GAZ_00144407 -->

    <owl:NamedIndividual rdf:about="http://purl.obolibrary.org/obo/GAZ_00144407">
        <obo:RO_0001025 rdf:resource="http://purl.obolibrary.org/obo/GAZ_00144376"/>
        <obo:IAO_0000115>A harbour of Rotterdam and the adjoining industrial area in the Netherlands. Being situated at the mouth of the rivers Rhine and Meuse with the hinterland consisting of the Netherlands, Germany, Belgium and partly France, Europoort is the world&apos;s busiest port and considered a major entry to Europe.</obo:IAO_0000115>
        <oboInOwl:hasOBONamespace>GAZ</oboInOwl:hasOBONamespace>
        <oboInOwl:id>GAZ:00144407</oboInOwl:id>
        <rdfs:label>Europoort</rdfs:label>
    </owl:NamedIndividual>
    


    <!-- http://purl.obolibrary.org/obo/GAZ_00144409 -->

    <owl:NamedIndividual rdf:about="http://purl.obolibrary.org/obo/GAZ_00144409">
        <rdf:type rdf:resource="http://purl.obolibrary.org/obo/ENVO_00000029"/>
        <obo:RO_0001025 rdf:resource="http://purl.obolibrary.org/obo/GAZ_00144376"/>
        <obo:IAO_0000115>A branch of the Rhine Delta that flows southwest from Nieuwegein.</obo:IAO_0000115>
        <oboInOwl:hasOBONamespace>GAZ</oboInOwl:hasOBONamespace>
        <oboInOwl:id>GAZ:00144409</oboInOwl:id>
        <rdfs:label>Enge IJssel</rdfs:label>
    </owl:NamedIndividual>
    


    <!-- http://purl.obolibrary.org/obo/GAZ_00144410 -->

    <owl:NamedIndividual rdf:about="http://purl.obolibrary.org/obo/GAZ_00144410">
        <rdf:type rdf:resource="http://purl.obolibrary.org/obo/ENVO_00000029"/>
        <obo:RO_0001025 rdf:resource="http://purl.obolibrary.org/obo/GAZ_00144376"/>
        <obo:IAO_0000115>A branch of the Rhine in the Dutch provinces of Gelderland and Overijssel. River IJssel flows from Westervoort, east of the city of Arnhem, until it discharges into the IJsselmeer until the 1932 completion of the Afsluitdijk known as the Zuiderzee, a North Sea inlet). River IJssel is one of the three major distributary branches into which the Rhine divides itself shortly after crossing the German-Dutch border, the other two being the rivers Nederrijn and Waal.</obo:IAO_0000115>
        <oboInOwl:hasOBONamespace>GAZ</oboInOwl:hasOBONamespace>
        <oboInOwl:id>GAZ:00144410</oboInOwl:id>
        <rdfs:label>IJssel</rdfs:label>
    </owl:NamedIndividual>
    


    <!-- http://purl.obolibrary.org/obo/GAZ_00144411 -->

    <owl:NamedIndividual rdf:about="http://purl.obolibrary.org/obo/GAZ_00144411">
        <obo:RO_0001025 rdf:resource="http://purl.obolibrary.org/obo/GAZ_00144376"/>
        <obo:IAO_0000115>The name of the Dutch part of River Rhine from the confluence at the town of Angeren of the cut-off Rhine bend of Oude Rijn and the Pannerdens Kanaal (which was dug to form the new connection between the Waal and Nederrijn branches). The city of Arnhem lies on the right (north) bank of the river Nederrijn, just past the branching-off of the River IJssel. River Nederrijn flows on to the city of Wijk bij Duurstede, from where it continues as the River Lek.</obo:IAO_0000115>
        <oboInOwl:hasOBONamespace>GAZ</oboInOwl:hasOBONamespace>
        <oboInOwl:id>GAZ:00144411</oboInOwl:id>
        <rdfs:label>Nederrijn</rdfs:label>
    </owl:NamedIndividual>
    


    <!-- http://purl.obolibrary.org/obo/GAZ_00144412 -->

    <owl:NamedIndividual rdf:about="http://purl.obolibrary.org/obo/GAZ_00144412">
        <obo:RO_0001025 rdf:resource="http://purl.obolibrary.org/obo/GAZ_00144376"/>
        <obo:IAO_0000115>A canal in the Netherlands that was dug between 1701 and 1709 to cut off a large, shallow bend of river Rhine and so improve river traffic and water regulation. The canal, now indistinguishable from a &quot;real&quot; river, forks off north from river Waal a few km past the point where the Bijlands Kanaal, a similar canal dug to cut off a Waal bend, ends. It flows past the towns of Pannerden (right bank), which gives the canal its name, and Angeren (left bank) and so north to the point where the old Rhine bend flows into it and the river continues to the sea as Nederrijn (Lower Rhine). The old Rhine bend, cut off at its upstream end, still exists and is called, unsurprisingly, Oude Rijn.</obo:IAO_0000115>
        <oboInOwl:hasOBONamespace>GAZ</oboInOwl:hasOBONamespace>
        <oboInOwl:id>GAZ:00144412</oboInOwl:id>
        <rdfs:label>Pannerdens Kanaal</rdfs:label>
    </owl:NamedIndividual>
    


    <!-- http://purl.obolibrary.org/obo/GAZ_00144413 -->

    <owl:NamedIndividual rdf:about="http://purl.obolibrary.org/obo/GAZ_00144413">
        <obo:RO_0001025 rdf:resource="http://purl.obolibrary.org/obo/GAZ_00144376"/>
        <obo:IAO_0000115>A river in Utrecht Province, the Netherlands. The Kromme Rijn splits off the Nederrijn-Lek main artery at the old town of Wijk bij Duurstede (called Dorestad before medieval times), after which it twists and turns through the province of Utrecht, past the towns of Cothen, Werkhoven, Odijk and Bunnik, and ends in the moat of the city of Utrecht.</obo:IAO_0000115>
        <oboInOwl:hasOBONamespace>GAZ</oboInOwl:hasOBONamespace>
        <oboInOwl:id>GAZ:00144413</oboInOwl:id>
        <rdfs:label>Kromme Rijn</rdfs:label>
    </owl:NamedIndividual>
    


    <!-- http://purl.obolibrary.org/obo/GAZ_00144414 -->

    <owl:NamedIndividual rdf:about="http://purl.obolibrary.org/obo/GAZ_00144414">
        <obo:RO_0001025 rdf:resource="http://purl.obolibrary.org/obo/GAZ_00144376"/>
        <obo:IAO_0000115>A short river in Utrecht Province, the Netherlands. It is the continuation of the Kromme Rijn (Crooked Rhine) after the city of Utrecht where both streams are part of the city&apos;s moat system. The Leidse Rijn ends at Harmelen. From here on it is called the Oude Rijn and drains into the North Sea at Katwijk.</obo:IAO_0000115>
        <oboInOwl:hasOBONamespace>GAZ</oboInOwl:hasOBONamespace>
        <oboInOwl:id>GAZ:00144414</oboInOwl:id>
        <rdfs:label>Leidse Rijn</rdfs:label>
    </owl:NamedIndividual>
    


    <!-- http://purl.obolibrary.org/obo/GAZ_00144415 -->

    <owl:NamedIndividual rdf:about="http://purl.obolibrary.org/obo/GAZ_00144415">
        <obo:RO_0001025 rdf:resource="http://purl.obolibrary.org/obo/GAZ_00144376"/>
        <obo:IAO_0000115>A river in the western Netherlands of some 60 km in length. It is the continuation of the Nederrijn after the Kromme Rijn branches off at the town of Wijk bij Duurstede. The main westbound waterway is hereafter called Lek River. The Nederrijn in turn is a distributary branch of river Rhine. Portions of the river form the boundary between the provinces of Utrecht and Gelderland, and between Utrecht and South Holland.</obo:IAO_0000115>
        <oboInOwl:hasOBONamespace>GAZ</oboInOwl:hasOBONamespace>
        <oboInOwl:id>GAZ:00144415</oboInOwl:id>
        <rdfs:label>Lek</rdfs:label>
    </owl:NamedIndividual>
    


    <!-- http://purl.obolibrary.org/obo/GAZ_00144416 -->

    <owl:NamedIndividual rdf:about="http://purl.obolibrary.org/obo/GAZ_00144416">
        <obo:RO_0001025 rdf:resource="http://purl.obolibrary.org/obo/GAZ_00144397"/>
        <obo:IAO_0000115>A river in the Betuwe that is over 100 km long, which makes it one of the longest rivers that flow entirely within the Netherlands. It starts near the village Doornenburg near the German border. It flows to Zoelen, a small village north of Tiel and from there on meanders through the Betuwe, to end in the Boven Merwede near Gorinchem. Until Geldermalsen the river is little more than a small, canalised stream. From Geldermalsen on however, it begins to look like a real river complete with dikes and small floodplains. The river was once a branch of the river Waal, being cut off at Tiel approximately in 1307.</obo:IAO_0000115>
        <oboInOwl:hasOBONamespace>GAZ</oboInOwl:hasOBONamespace>
        <oboInOwl:id>GAZ:00144416</oboInOwl:id>
        <rdfs:label>Linge</rdfs:label>
    </owl:NamedIndividual>
    


    <!-- http://purl.obolibrary.org/obo/GAZ_00144418 -->

    <owl:NamedIndividual rdf:about="http://purl.obolibrary.org/obo/GAZ_00144418">
        <obo:RO_0001025 rdf:resource="http://purl.obolibrary.org/obo/GAZ_00144393"/>
        <obo:IAO_0000115>A storm surge barrier in the Nieuwe Waterweg waterway located between the towns of Hoek van Holland and Maassluis, Netherlands. Completed in 1997.</obo:IAO_0000115>
        <oboInOwl:hasOBONamespace>GAZ</oboInOwl:hasOBONamespace>
        <oboInOwl:id>GAZ:00144418</oboInOwl:id>
        <rdfs:label>Maeslantkering</rdfs:label>
    </owl:NamedIndividual>
    


    <!-- http://purl.obolibrary.org/obo/GAZ_00144419 -->

    <owl:NamedIndividual rdf:about="http://purl.obolibrary.org/obo/GAZ_00144419">
        <obo:RO_0001025 rdf:resource="http://purl.obolibrary.org/obo/GAZ_00144376"/>
        <obo:IAO_0000115>The name of several interconnected stretches of river in The Netherlands, all part of the Rhine-Meuse-Scheldt delta. The Meuse river joins the Waal at Woudrichem to form the Boven Merwede (Upper Merwede). A few km downstream it splits into the Beneden Merwede (Lower Merwede) on the right and the Nieuwe Merwede (New Merwede) on the left. All these rivers are tidal. The Nieuwe Merwede joins the Bergse Maas near Lage Zwaluwe to form the Hollands Diep estuary, and separates the Island of Dordrecht from the Biesbosch National Park. The Beneden Merwede splits into the Noord River and Oude Maas near Papendrecht.</obo:IAO_0000115>
        <oboInOwl:hasOBONamespace>GAZ</oboInOwl:hasOBONamespace>
        <oboInOwl:id>GAZ:00144419</oboInOwl:id>
        <rdfs:label>Merwede</rdfs:label>
    </owl:NamedIndividual>
    


    <!-- http://purl.obolibrary.org/obo/GAZ_00144420 -->

    <owl:NamedIndividual rdf:about="http://purl.obolibrary.org/obo/GAZ_00144420">
        <obo:RO_0001025 rdf:resource="http://purl.obolibrary.org/obo/GAZ_00090210"/>
        <obo:IAO_0000115>An artificial island in the Netherlands in the province of Zeeland, halfway between Noord-Beveland and Schouwen-Duiveland in the Oosterschelde. It was constructed to facilitate the construction of the Oosterscheldedam.</obo:IAO_0000115>
        <oboInOwl:hasOBONamespace>GAZ</oboInOwl:hasOBONamespace>
        <oboInOwl:id>GAZ:00144420</oboInOwl:id>
        <rdfs:label>Neeltje-Jans</rdfs:label>
    </owl:NamedIndividual>
    


    <!-- http://purl.obolibrary.org/obo/GAZ_00144421 -->

    <owl:NamedIndividual rdf:about="http://purl.obolibrary.org/obo/GAZ_00144421">
        <obo:RO_0001025 rdf:resource="http://purl.obolibrary.org/obo/GAZ_00144376"/>
        <obo:IAO_0000115>A short tidal river in South Holland in the Netherlands. It starts at the city of Dordrecht where the Beneden Merwede river forks into the Oude Maas and the Noord. It joins the Lek at the city of Ridderkerk and Kinderdijk, and the combined stream is thereafter known as the Nieuwe Maas. The Noord River separates IJsselmonde island from Alblasserwaard mainland to the east. There are two connections between them.</obo:IAO_0000115>
        <oboInOwl:hasOBONamespace>GAZ</oboInOwl:hasOBONamespace>
        <oboInOwl:id>GAZ:00144421</oboInOwl:id>
        <rdfs:label>Noord River</rdfs:label>
    </owl:NamedIndividual>
    


    <!-- http://purl.obolibrary.org/obo/GAZ_00144423 -->

    <owl:NamedIndividual rdf:about="http://purl.obolibrary.org/obo/GAZ_00144423">
        <obo:RO_0001025 rdf:resource="http://purl.obolibrary.org/obo/GAZ_00090210"/>
        <obo:IAO_0000115>An artificial storm barrier between the islands Schouwen-Duiveland and Noord-Beveland. Completed 1986.</obo:IAO_0000115>
        <oboInOwl:hasOBONamespace>GAZ</oboInOwl:hasOBONamespace>
        <oboInOwl:id>GAZ:00144423</oboInOwl:id>
        <rdfs:label>Oosterscheldekering</rdfs:label>
    </owl:NamedIndividual>
    


    <!-- http://purl.obolibrary.org/obo/GAZ_00144425 -->

    <owl:NamedIndividual rdf:about="http://purl.obolibrary.org/obo/GAZ_00144425">
        <obo:RO_0001025 rdf:resource="http://purl.obolibrary.org/obo/GAZ_00144376"/>
        <obo:IAO_0000115>A canal in the Netherlands, in the province of South Holland. It starts at the Oude Rijn at Leiden and joins the Delfshavense Schie canal at Delft. Places along its banks include Voorschoten, Leidschendam, Voorburg, The Hague and Ryswick. The canal was dug in 47 AD.</obo:IAO_0000115>
        <oboInOwl:hasOBONamespace>GAZ</oboInOwl:hasOBONamespace>
        <oboInOwl:id>GAZ:00144425</oboInOwl:id>
        <rdfs:label>Vliet</rdfs:label>
    </owl:NamedIndividual>
    


    <!-- http://purl.obolibrary.org/obo/GAZ_00179289 -->

    <owl:NamedIndividual rdf:about="http://purl.obolibrary.org/obo/GAZ_00179289">
        <obo:RO_0001025 rdf:resource="http://purl.obolibrary.org/obo/GAZ_00004124"/>
        <obo:IAO_0000115>A natural park near Purkersdorf in the Vienna Woods (Wienerwald), Austria.</obo:IAO_0000115>
        <oboInOwl:hasOBONamespace>GAZ</oboInOwl:hasOBONamespace>
        <oboInOwl:id>GAZ:00179289</oboInOwl:id>
        <rdfs:label>Sandstein-Wienerwald Natural Park</rdfs:label>
    </owl:NamedIndividual>
    


    <!-- http://purl.obolibrary.org/obo/GAZ_00179294 -->

    <owl:NamedIndividual rdf:about="http://purl.obolibrary.org/obo/GAZ_00179294">
        <obo:RO_0001025 rdf:resource="http://purl.obolibrary.org/obo/GAZ_00101709"/>
        <obo:IAO_0000115>A cave.</obo:IAO_0000115>
        <oboInOwl:hasOBONamespace>GAZ</oboInOwl:hasOBONamespace>
        <oboInOwl:id>GAZ:00179294</oboInOwl:id>
        <rdfs:label>Steinbruckenhohle</rdfs:label>
    </owl:NamedIndividual>
    


    <!-- http://purl.obolibrary.org/obo/GAZ_00179296 -->

    <owl:NamedIndividual rdf:about="http://purl.obolibrary.org/obo/GAZ_00179296">
        <obo:RO_0001025 rdf:resource="http://purl.obolibrary.org/obo/GAZ_00056784"/>
        <obo:IAO_0000115>A mountain in the main chain of the Alps in the district of Kaprun, Salzburg, Austria.</obo:IAO_0000115>
        <oboInOwl:hasOBONamespace>GAZ</oboInOwl:hasOBONamespace>
        <oboInOwl:id>GAZ:00179296</oboInOwl:id>
        <rdfs:label>Kitzsteinhorn</rdfs:label>
    </owl:NamedIndividual>
    


    <!-- http://purl.obolibrary.org/obo/GAZ_00179297 -->

    <owl:NamedIndividual rdf:about="http://purl.obolibrary.org/obo/GAZ_00179297">
        <obo:RO_0001025 rdf:resource="http://purl.obolibrary.org/obo/GAZ_00179296"/>
        <obo:IAO_0000115>A glacier.</obo:IAO_0000115>
        <oboInOwl:hasOBONamespace>GAZ</oboInOwl:hasOBONamespace>
        <oboInOwl:id>GAZ:00179297</oboInOwl:id>
        <rdfs:label>Maurerkees Glacier</rdfs:label>
    </owl:NamedIndividual>
    


    <!-- http://purl.obolibrary.org/obo/GAZ_00179298 -->

    <owl:NamedIndividual rdf:about="http://purl.obolibrary.org/obo/GAZ_00179298">
        <obo:RO_0001025 rdf:resource="http://purl.obolibrary.org/obo/GAZ_00179296"/>
        <obo:IAO_0000115>A glacier.</obo:IAO_0000115>
        <oboInOwl:hasOBONamespace>GAZ</oboInOwl:hasOBONamespace>
        <oboInOwl:id>GAZ:00179298</oboInOwl:id>
        <rdfs:label>Schmiedingerkees Glacier</rdfs:label>
    </owl:NamedIndividual>
    


    <!-- http://purl.obolibrary.org/obo/GAZ_00179752 -->

    <owl:NamedIndividual rdf:about="http://purl.obolibrary.org/obo/GAZ_00179752">
        <obo:RO_0001025 rdf:resource="http://purl.obolibrary.org/obo/GAZ_00144376"/>
        <oboInOwl:hasOBONamespace>GAZ</oboInOwl:hasOBONamespace>
        <oboInOwl:id>GAZ:00179752</oboInOwl:id>
        <rdfs:label>Scheldt Estuary</rdfs:label>
    </owl:NamedIndividual>
    


    <!-- http://purl.obolibrary.org/obo/GAZ_00261031 -->

    <owl:NamedIndividual rdf:about="http://purl.obolibrary.org/obo/GAZ_00261031">
        <rdf:type rdf:resource="http://purl.obolibrary.org/obo/ENVO_00000080"/>
        <obo:RO_0001025 rdf:resource="http://purl.obolibrary.org/obo/GAZ_00056784"/>
        <obo:IAO_0000115>A mountain group within the Hohe Tauern.</obo:IAO_0000115>
        <oboInOwl:hasOBONamespace>GAZ</oboInOwl:hasOBONamespace>
        <oboInOwl:id>GAZ:00261031</oboInOwl:id>
        <rdfs:label>Venediger Group</rdfs:label>
    </owl:NamedIndividual>
    


    <!-- http://purl.obolibrary.org/obo/GAZ_00261032 -->

    <owl:NamedIndividual rdf:about="http://purl.obolibrary.org/obo/GAZ_00261032">
        <rdf:type rdf:resource="http://purl.obolibrary.org/obo/ENVO_00000080"/>
        <obo:RO_0001025 rdf:resource="http://purl.obolibrary.org/obo/GAZ_00056784"/>
        <obo:IAO_0000115>A mountain group within the Hohe Tauern.</obo:IAO_0000115>
        <oboInOwl:hasOBONamespace>GAZ</oboInOwl:hasOBONamespace>
        <oboInOwl:id>GAZ:00261032</oboInOwl:id>
        <rdfs:label>Granatspitz Group</rdfs:label>
    </owl:NamedIndividual>
    


    <!-- http://purl.obolibrary.org/obo/GAZ_00261033 -->

    <owl:NamedIndividual rdf:about="http://purl.obolibrary.org/obo/GAZ_00261033">
        <rdf:type rdf:resource="http://purl.obolibrary.org/obo/ENVO_00000080"/>
        <obo:RO_0001025 rdf:resource="http://purl.obolibrary.org/obo/GAZ_00056784"/>
        <obo:IAO_0000115>A mountain group within the Hohe Tauern.</obo:IAO_0000115>
        <oboInOwl:hasOBONamespace>GAZ</oboInOwl:hasOBONamespace>
        <oboInOwl:id>GAZ:00261033</oboInOwl:id>
        <rdfs:label>Glockner Group</rdfs:label>
    </owl:NamedIndividual>
    


    <!-- http://purl.obolibrary.org/obo/GAZ_00261034 -->

    <owl:NamedIndividual rdf:about="http://purl.obolibrary.org/obo/GAZ_00261034">
        <rdf:type rdf:resource="http://purl.obolibrary.org/obo/ENVO_00000080"/>
        <obo:RO_0001025 rdf:resource="http://purl.obolibrary.org/obo/GAZ_00056784"/>
        <obo:IAO_0000115>A mountain group within the Hohe Tauern.</obo:IAO_0000115>
        <oboInOwl:hasOBONamespace>GAZ</oboInOwl:hasOBONamespace>
        <oboInOwl:id>GAZ:00261034</oboInOwl:id>
        <rdfs:label>Goldberg Group</rdfs:label>
    </owl:NamedIndividual>
    


    <!-- http://purl.obolibrary.org/obo/GAZ_00261035 -->

    <owl:NamedIndividual rdf:about="http://purl.obolibrary.org/obo/GAZ_00261035">
        <rdf:type rdf:resource="http://purl.obolibrary.org/obo/ENVO_00000080"/>
        <obo:RO_0001025 rdf:resource="http://purl.obolibrary.org/obo/GAZ_00056784"/>
        <obo:IAO_0000115>A mountain group within the Hohe Tauern.</obo:IAO_0000115>
        <oboInOwl:hasOBONamespace>GAZ</oboInOwl:hasOBONamespace>
        <oboInOwl:id>GAZ:00261035</oboInOwl:id>
        <rdfs:label>Ankogel Group</rdfs:label>
    </owl:NamedIndividual>
    


    <!-- http://purl.obolibrary.org/obo/GAZ_00261036 -->

    <owl:NamedIndividual rdf:about="http://purl.obolibrary.org/obo/GAZ_00261036">
        <rdf:type rdf:resource="http://purl.obolibrary.org/obo/ENVO_00000080"/>
        <obo:RO_0001025 rdf:resource="http://purl.obolibrary.org/obo/GAZ_00056784"/>
        <obo:IAO_0000115>A mountain group within the Hohe Tauern.</obo:IAO_0000115>
        <oboInOwl:hasOBONamespace>GAZ</oboInOwl:hasOBONamespace>
        <oboInOwl:id>GAZ:00261036</oboInOwl:id>
        <rdfs:label>Hafner Group</rdfs:label>
    </owl:NamedIndividual>
    


    <!-- http://purl.obolibrary.org/obo/GAZ_00261037 -->

    <owl:NamedIndividual rdf:about="http://purl.obolibrary.org/obo/GAZ_00261037">
        <rdf:type rdf:resource="http://purl.obolibrary.org/obo/ENVO_00000080"/>
        <obo:RO_0001025 rdf:resource="http://purl.obolibrary.org/obo/GAZ_00056784"/>
        <obo:IAO_0000115>A mountain group within the Hohe Tauern.</obo:IAO_0000115>
        <oboInOwl:hasOBONamespace>GAZ</oboInOwl:hasOBONamespace>
        <oboInOwl:id>GAZ:00261037</oboInOwl:id>
        <rdfs:label>Lasorling Groups</rdfs:label>
    </owl:NamedIndividual>
    


    <!-- http://purl.obolibrary.org/obo/GAZ_00261038 -->

    <owl:NamedIndividual rdf:about="http://purl.obolibrary.org/obo/GAZ_00261038">
        <rdf:type rdf:resource="http://purl.obolibrary.org/obo/ENVO_00000080"/>
        <obo:RO_0001025 rdf:resource="http://purl.obolibrary.org/obo/GAZ_00056784"/>
        <obo:IAO_0000115>A mountain group within the Hohe Tauern.</obo:IAO_0000115>
        <oboInOwl:hasOBONamespace>GAZ</oboInOwl:hasOBONamespace>
        <oboInOwl:id>GAZ:00261038</oboInOwl:id>
        <rdfs:label>Rieserferner Group</rdfs:label>
    </owl:NamedIndividual>
    


    <!-- http://purl.obolibrary.org/obo/GAZ_00261039 -->

    <owl:NamedIndividual rdf:about="http://purl.obolibrary.org/obo/GAZ_00261039">
        <rdf:type rdf:resource="http://purl.obolibrary.org/obo/ENVO_00000080"/>
        <obo:RO_0001025 rdf:resource="http://purl.obolibrary.org/obo/GAZ_00056784"/>
        <obo:IAO_0000115>A mountain group within the Hohe Tauern.</obo:IAO_0000115>
        <oboInOwl:hasOBONamespace>GAZ</oboInOwl:hasOBONamespace>
        <oboInOwl:id>GAZ:00261039</oboInOwl:id>
        <rdfs:label>Schober Group</rdfs:label>
    </owl:NamedIndividual>
    


    <!-- http://purl.obolibrary.org/obo/GAZ_00261040 -->

    <owl:NamedIndividual rdf:about="http://purl.obolibrary.org/obo/GAZ_00261040">
        <rdf:type rdf:resource="http://purl.obolibrary.org/obo/ENVO_00000080"/>
        <obo:RO_0001025 rdf:resource="http://purl.obolibrary.org/obo/GAZ_00056784"/>
        <obo:IAO_0000115>A mountain group within the Hohe Tauern.</obo:IAO_0000115>
        <oboInOwl:hasOBONamespace>GAZ</oboInOwl:hasOBONamespace>
        <oboInOwl:id>GAZ:00261040</oboInOwl:id>
        <rdfs:label>Kreuzeck Group</rdfs:label>
    </owl:NamedIndividual>
    


    <!-- http://purl.obolibrary.org/obo/GAZ_00324438 -->

    <owl:NamedIndividual rdf:about="http://purl.obolibrary.org/obo/GAZ_00324438">
        <obo:IAO_0000115>A river.</obo:IAO_0000115>
        <oboInOwl:hasOBONamespace>GAZ</oboInOwl:hasOBONamespace>
        <oboInOwl:id>GAZ:00324438</oboInOwl:id>
        <rdfs:label>Zwarte Water</rdfs:label>
    </owl:NamedIndividual>
    


    <!-- http://purl.obolibrary.org/obo/GAZ_00324603 -->

    <owl:NamedIndividual rdf:about="http://purl.obolibrary.org/obo/GAZ_00324603">
        <obo:RO_0001025 rdf:resource="http://purl.obolibrary.org/obo/GAZ_00144376"/>
        <obo:IAO_0000115>A branch of the River Rhine in the Dutch province of Utrecht. The Vecht originates in the city of Utrecht, where the Kromme Rijn stream forks into two branches: the Leidse Rijn/Oude Rijn branch to the west and the Vecht to the north. The Vecht twists and turns north past the towns and villages of Maarssen, Breukelen and Nigtevecht, crosses the border into the province of North Holland, passes the town of Weesp and discharges into the Markermeer (Lake Marken, formerly the Zuiderzee) at Muiden. The Amsterdam-Rijnkanaal (Amsterdam-Rhine Canal) was dug in the Vecht basin.</obo:IAO_0000115>
        <oboInOwl:hasOBONamespace>GAZ</oboInOwl:hasOBONamespace>
        <oboInOwl:id>GAZ:00324603</oboInOwl:id>
        <rdfs:label>Utrechtse Vecht</rdfs:label>
    </owl:NamedIndividual>
    


    <!-- http://purl.obolibrary.org/obo/GAZ_00324756 -->

    <owl:NamedIndividual rdf:about="http://purl.obolibrary.org/obo/GAZ_00324756">
        <obo:IAO_0000115>A river.</obo:IAO_0000115>
        <oboInOwl:hasOBONamespace>GAZ</oboInOwl:hasOBONamespace>
        <oboInOwl:id>GAZ:00324756</oboInOwl:id>
        <rdfs:label>Sint-Jansbeek</rdfs:label>
    </owl:NamedIndividual>
    


    <!-- http://purl.obolibrary.org/obo/GAZ_00325162 -->

    <owl:NamedIndividual rdf:about="http://purl.obolibrary.org/obo/GAZ_00325162">
        <obo:RO_0001025 rdf:resource="http://purl.obolibrary.org/obo/GAZ_00144362"/>
        <obo:IAO_0000115>A canal in the Netherlands that connects Antwerp with the Volkerak, and thereby the Scheldt with the Rhine. The Scheldt-Rhine canal includes the Eendracht.</obo:IAO_0000115>
        <oboInOwl:hasOBONamespace>GAZ</oboInOwl:hasOBONamespace>
        <oboInOwl:id>GAZ:00325162</oboInOwl:id>
        <rdfs:label>Schelde-Rijnkanaal</rdfs:label>
    </owl:NamedIndividual>
    


    <!-- http://purl.obolibrary.org/obo/GAZ_00325244 -->

    <owl:NamedIndividual rdf:about="http://purl.obolibrary.org/obo/GAZ_00325244">
        <obo:RO_0001025 rdf:resource="http://purl.obolibrary.org/obo/GAZ_00090210"/>
        <obo:IAO_0000115>A lake.</obo:IAO_0000115>
        <oboInOwl:hasOBONamespace>GAZ</oboInOwl:hasOBONamespace>
        <oboInOwl:id>GAZ:00325244</oboInOwl:id>
        <rdfs:label>Markiezaatsmeer</rdfs:label>
    </owl:NamedIndividual>
    


    <!-- http://purl.obolibrary.org/obo/GAZ_00325310 -->

    <owl:NamedIndividual rdf:about="http://purl.obolibrary.org/obo/GAZ_00325310">
        <obo:RO_0001025 rdf:resource="http://purl.obolibrary.org/obo/GAZ_00090211"/>
        <oboInOwl:hasOBONamespace>GAZ</oboInOwl:hasOBONamespace>
        <oboInOwl:id>GAZ:00325310</oboInOwl:id>
        <rdfs:label>Brabantse Biesbosch</rdfs:label>
    </owl:NamedIndividual>
    


    <!-- http://purl.obolibrary.org/obo/GAZ_00325315 -->

    <owl:NamedIndividual rdf:about="http://purl.obolibrary.org/obo/GAZ_00325315">
        <obo:IAO_0000115>A river.</obo:IAO_0000115>
        <oboInOwl:hasOBONamespace>GAZ</oboInOwl:hasOBONamespace>
        <oboInOwl:id>GAZ:00325315</oboInOwl:id>
        <rdfs:label>Gat van den Kleinen Hil</rdfs:label>
    </owl:NamedIndividual>
    


    <!-- http://purl.obolibrary.org/obo/GAZ_00325317 -->

    <owl:NamedIndividual rdf:about="http://purl.obolibrary.org/obo/GAZ_00325317">
        <obo:RO_0001025 rdf:resource="http://purl.obolibrary.org/obo/GAZ_00144376"/>
        <obo:IAO_0000115>An estuary. Located between the island Goeree-Overflakkee to the north-west and the Dutch mainland to the south and east. The western part of the Volkerak is also called Krammer.</obo:IAO_0000115>
        <oboInOwl:hasOBONamespace>GAZ</oboInOwl:hasOBONamespace>
        <oboInOwl:id>GAZ:00325317</oboInOwl:id>
        <rdfs:label>Volkerak</rdfs:label>
    </owl:NamedIndividual>
    


    <!-- http://purl.obolibrary.org/obo/GAZ_00325494 -->

    <owl:NamedIndividual rdf:about="http://purl.obolibrary.org/obo/GAZ_00325494">
        <obo:IAO_0000115>A river.</obo:IAO_0000115>
        <oboInOwl:hasOBONamespace>GAZ</oboInOwl:hasOBONamespace>
        <oboInOwl:id>GAZ:00325494</oboInOwl:id>
        <rdfs:label>Amstel</rdfs:label>
    </owl:NamedIndividual>
    


    <!-- http://purl.obolibrary.org/obo/GAZ_00325495 -->

    <owl:NamedIndividual rdf:about="http://purl.obolibrary.org/obo/GAZ_00325495">
        <obo:RO_0001025 rdf:resource="http://purl.obolibrary.org/obo/GAZ_00325494"/>
        <obo:IAO_0000115>An island.</obo:IAO_0000115>
        <oboInOwl:hasOBONamespace>GAZ</oboInOwl:hasOBONamespace>
        <oboInOwl:id>GAZ:00325495</oboInOwl:id>
        <rdfs:label>Amsteleiland</rdfs:label>
    </owl:NamedIndividual>
    


    <!-- http://purl.obolibrary.org/obo/GAZ_00325590 -->

    <owl:NamedIndividual rdf:about="http://purl.obolibrary.org/obo/GAZ_00325590">
        <obo:RO_0001025 rdf:resource="http://purl.obolibrary.org/obo/GAZ_00325627"/>
        <obo:IAO_0000115>A harbor.</obo:IAO_0000115>
        <oboInOwl:hasOBONamespace>GAZ</oboInOwl:hasOBONamespace>
        <oboInOwl:id>GAZ:00325590</oboInOwl:id>
        <rdfs:label>Afrikahaven</rdfs:label>
    </owl:NamedIndividual>
    


    <!-- http://purl.obolibrary.org/obo/GAZ_00325627 -->

    <owl:NamedIndividual rdf:about="http://purl.obolibrary.org/obo/GAZ_00325627">
        <obo:IAO_0000115>A harbor.</obo:IAO_0000115>
        <oboInOwl:hasOBONamespace>GAZ</oboInOwl:hasOBONamespace>
        <oboInOwl:id>GAZ:00325627</oboInOwl:id>
        <rdfs:label>Haven van Amsterdam</rdfs:label>
    </owl:NamedIndividual>
    


    <!-- http://purl.obolibrary.org/obo/GAZ_00325628 -->

    <owl:NamedIndividual rdf:about="http://purl.obolibrary.org/obo/GAZ_00325628">
        <obo:RO_0001025 rdf:resource="http://purl.obolibrary.org/obo/GAZ_00325627"/>
        <obo:IAO_0000115>A harbor.</obo:IAO_0000115>
        <oboInOwl:hasOBONamespace>GAZ</oboInOwl:hasOBONamespace>
        <oboInOwl:id>GAZ:00325628</oboInOwl:id>
        <rdfs:label>Amerikahaven</rdfs:label>
    </owl:NamedIndividual>
    


    <!-- http://purl.obolibrary.org/obo/GAZ_00325629 -->

    <owl:NamedIndividual rdf:about="http://purl.obolibrary.org/obo/GAZ_00325629">
        <obo:RO_0001025 rdf:resource="http://purl.obolibrary.org/obo/GAZ_00325627"/>
        <obo:IAO_0000115>A harbor.</obo:IAO_0000115>
        <oboInOwl:hasOBONamespace>GAZ</oboInOwl:hasOBONamespace>
        <oboInOwl:id>GAZ:00325629</oboInOwl:id>
        <rdfs:label>Westhaven</rdfs:label>
    </owl:NamedIndividual>
    


    <!-- http://purl.obolibrary.org/obo/GAZ_00325630 -->

    <owl:NamedIndividual rdf:about="http://purl.obolibrary.org/obo/GAZ_00325630">
        <obo:RO_0001025 rdf:resource="http://purl.obolibrary.org/obo/GAZ_00325627"/>
        <obo:IAO_0000115>A harbor.</obo:IAO_0000115>
        <oboInOwl:hasOBONamespace>GAZ</oboInOwl:hasOBONamespace>
        <oboInOwl:id>GAZ:00325630</oboInOwl:id>
        <rdfs:label>Jan van Riebeeckhaven</rdfs:label>
    </owl:NamedIndividual>
    


    <!-- http://purl.obolibrary.org/obo/GAZ_00325631 -->

    <owl:NamedIndividual rdf:about="http://purl.obolibrary.org/obo/GAZ_00325631">
        <obo:RO_0001025 rdf:resource="http://purl.obolibrary.org/obo/GAZ_00325627"/>
        <obo:IAO_0000115>A harbor.</obo:IAO_0000115>
        <oboInOwl:hasOBONamespace>GAZ</oboInOwl:hasOBONamespace>
        <oboInOwl:id>GAZ:00325631</oboInOwl:id>
        <rdfs:label>Petroleumhaven</rdfs:label>
    </owl:NamedIndividual>
    


    <!-- http://purl.obolibrary.org/obo/GAZ_00325632 -->

    <owl:NamedIndividual rdf:about="http://purl.obolibrary.org/obo/GAZ_00325632">
        <obo:RO_0001025 rdf:resource="http://purl.obolibrary.org/obo/GAZ_00325627"/>
        <obo:IAO_0000115>A harbor.</obo:IAO_0000115>
        <oboInOwl:hasOBONamespace>GAZ</oboInOwl:hasOBONamespace>
        <oboInOwl:id>GAZ:00325632</oboInOwl:id>
        <rdfs:label>Coenhaven</rdfs:label>
    </owl:NamedIndividual>
    


    <!-- http://purl.obolibrary.org/obo/GAZ_00325633 -->

    <owl:NamedIndividual rdf:about="http://purl.obolibrary.org/obo/GAZ_00325633">
        <obo:RO_0001025 rdf:resource="http://purl.obolibrary.org/obo/GAZ_00325627"/>
        <obo:IAO_0000115>A harbor.</obo:IAO_0000115>
        <oboInOwl:hasOBONamespace>GAZ</oboInOwl:hasOBONamespace>
        <oboInOwl:id>GAZ:00325633</oboInOwl:id>
        <rdfs:label>Mercuriushaven</rdfs:label>
    </owl:NamedIndividual>
    


    <!-- http://purl.obolibrary.org/obo/GAZ_00325634 -->

    <owl:NamedIndividual rdf:about="http://purl.obolibrary.org/obo/GAZ_00325634">
        <obo:RO_0001025 rdf:resource="http://purl.obolibrary.org/obo/GAZ_00325627"/>
        <obo:IAO_0000115>A harbor.</obo:IAO_0000115>
        <oboInOwl:hasOBONamespace>GAZ</oboInOwl:hasOBONamespace>
        <oboInOwl:id>GAZ:00325634</oboInOwl:id>
        <rdfs:label>Houthaven</rdfs:label>
    </owl:NamedIndividual>
    


    <!-- http://purl.obolibrary.org/obo/GAZ_00325635 -->

    <owl:NamedIndividual rdf:about="http://purl.obolibrary.org/obo/GAZ_00325635">
        <obo:RO_0001025 rdf:resource="http://purl.obolibrary.org/obo/GAZ_00325627"/>
        <obo:IAO_0000115>A harbor.</obo:IAO_0000115>
        <oboInOwl:hasOBONamespace>GAZ</oboInOwl:hasOBONamespace>
        <oboInOwl:id>GAZ:00325635</oboInOwl:id>
        <rdfs:label>Oostelijk Havengebied</rdfs:label>
    </owl:NamedIndividual>
    


    <!-- http://purl.obolibrary.org/obo/GAZ_00325644 -->

    <owl:NamedIndividual rdf:about="http://purl.obolibrary.org/obo/GAZ_00325644">
        <obo:RO_0001025 rdf:resource="http://purl.obolibrary.org/obo/GAZ_00325633"/>
        <obo:IAO_0000115>A harbor.</obo:IAO_0000115>
        <oboInOwl:hasOBONamespace>GAZ</oboInOwl:hasOBONamespace>
        <oboInOwl:id>GAZ:00325644</oboInOwl:id>
        <rdfs:label>Minervahaven</rdfs:label>
    </owl:NamedIndividual>
    


    <!-- http://purl.obolibrary.org/obo/GAZ_00325649 -->

    <owl:NamedIndividual rdf:about="http://purl.obolibrary.org/obo/GAZ_00325649">
        <obo:IAO_0000115>A body of water.</obo:IAO_0000115>
        <oboInOwl:hasOBONamespace>GAZ</oboInOwl:hasOBONamespace>
        <oboInOwl:id>GAZ:00325649</oboInOwl:id>
        <rdfs:label>Oosterdok</rdfs:label>
    </owl:NamedIndividual>
    


    <!-- http://purl.obolibrary.org/obo/GAZ_00325652 -->

    <owl:NamedIndividual rdf:about="http://purl.obolibrary.org/obo/GAZ_00325652">
        <obo:RO_0001025 rdf:resource="http://purl.obolibrary.org/obo/GAZ_00325635"/>
        <obo:IAO_0000115>A Canal.</obo:IAO_0000115>
        <oboInOwl:hasOBONamespace>GAZ</oboInOwl:hasOBONamespace>
        <oboInOwl:id>GAZ:00325652</oboInOwl:id>
        <rdfs:label>Spoorwegbassin</rdfs:label>
    </owl:NamedIndividual>
    


    <!-- http://purl.obolibrary.org/obo/GAZ_00325655 -->

    <owl:NamedIndividual rdf:about="http://purl.obolibrary.org/obo/GAZ_00325655">
        <obo:RO_0001025 rdf:resource="http://purl.obolibrary.org/obo/GAZ_00058902"/>
        <obo:IAO_0000115>A body of water.</obo:IAO_0000115>
        <oboInOwl:hasOBONamespace>GAZ</oboInOwl:hasOBONamespace>
        <oboInOwl:id>GAZ:00325655</oboInOwl:id>
        <rdfs:label>Westerdok</rdfs:label>
    </owl:NamedIndividual>
    


    <!-- http://purl.obolibrary.org/obo/GAZ_00325986 -->

    <owl:NamedIndividual rdf:about="http://purl.obolibrary.org/obo/GAZ_00325986">
        <obo:RO_0001025 rdf:resource="http://purl.obolibrary.org/obo/GAZ_00021224"/>
        <obo:IAO_0000115>An area.</obo:IAO_0000115>
        <oboInOwl:hasOBONamespace>GAZ</oboInOwl:hasOBONamespace>
        <oboInOwl:id>GAZ:00325986</oboInOwl:id>
        <rdfs:label>Zak van Zuid-Beveland</rdfs:label>
    </owl:NamedIndividual>
    


    <!-- http://purl.obolibrary.org/obo/GAZ_00326037 -->

    <owl:NamedIndividual rdf:about="http://purl.obolibrary.org/obo/GAZ_00326037">
        <obo:IAO_0000115>A river.</obo:IAO_0000115>
        <oboInOwl:hasOBONamespace>GAZ</oboInOwl:hasOBONamespace>
        <oboInOwl:id>GAZ:00326037</oboInOwl:id>
        <rdfs:label>Bethlehemschebeek</rdfs:label>
    </owl:NamedIndividual>
    


    <!-- http://purl.obolibrary.org/obo/GAZ_00326084 -->

    <owl:NamedIndividual rdf:about="http://purl.obolibrary.org/obo/GAZ_00326084">
        <obo:IAO_0000115>A river.</obo:IAO_0000115>
        <oboInOwl:hasOBONamespace>GAZ</oboInOwl:hasOBONamespace>
        <oboInOwl:id>GAZ:00326084</oboInOwl:id>
        <rdfs:label>Drekkersstrang</rdfs:label>
    </owl:NamedIndividual>
    


    <!-- http://purl.obolibrary.org/obo/GAZ_00326196 -->

    <owl:NamedIndividual rdf:about="http://purl.obolibrary.org/obo/GAZ_00326196">
        <obo:IAO_0000115>A Canal.</obo:IAO_0000115>
        <oboInOwl:hasOBONamespace>GAZ</oboInOwl:hasOBONamespace>
        <oboInOwl:id>GAZ:00326196</oboInOwl:id>
        <rdfs:label>Witte Singel</rdfs:label>
    </owl:NamedIndividual>
    


    <!-- http://purl.obolibrary.org/obo/GAZ_00326332 -->

    <owl:NamedIndividual rdf:about="http://purl.obolibrary.org/obo/GAZ_00326332">
        <obo:RO_0001025 rdf:resource="http://purl.obolibrary.org/obo/GAZ_00144393"/>
        <obo:IAO_0000115>A harbor.</obo:IAO_0000115>
        <oboInOwl:hasOBONamespace>GAZ</oboInOwl:hasOBONamespace>
        <oboInOwl:id>GAZ:00326332</oboInOwl:id>
        <rdfs:label>Berghaven</rdfs:label>
    </owl:NamedIndividual>
    


    <!-- http://purl.obolibrary.org/obo/GAZ_00326381 -->

    <owl:NamedIndividual rdf:about="http://purl.obolibrary.org/obo/GAZ_00326381">
        <obo:IAO_0000115>A dam.</obo:IAO_0000115>
        <oboInOwl:hasOBONamespace>GAZ</oboInOwl:hasOBONamespace>
        <oboInOwl:id>GAZ:00326381</oboInOwl:id>
        <rdfs:label>Brielse Maasdam</rdfs:label>
    </owl:NamedIndividual>
    


    <!-- http://purl.obolibrary.org/obo/GAZ_00326382 -->

    <owl:NamedIndividual rdf:about="http://purl.obolibrary.org/obo/GAZ_00326382">
        <obo:IAO_0000115>A dam.</obo:IAO_0000115>
        <oboInOwl:hasOBONamespace>GAZ</oboInOwl:hasOBONamespace>
        <oboInOwl:id>GAZ:00326382</oboInOwl:id>
        <rdfs:label>Brielse Gatdam</rdfs:label>
    </owl:NamedIndividual>
    


    <!-- http://purl.obolibrary.org/obo/GAZ_00326402 -->

    <owl:NamedIndividual rdf:about="http://purl.obolibrary.org/obo/GAZ_00326402">
        <obo:IAO_0000115>A Canal.</obo:IAO_0000115>
        <oboInOwl:hasOBONamespace>GAZ</oboInOwl:hasOBONamespace>
        <oboInOwl:id>GAZ:00326402</oboInOwl:id>
        <rdfs:label>Kantoorgracht</rdfs:label>
    </owl:NamedIndividual>
    


    <!-- http://purl.obolibrary.org/obo/GAZ_00326422 -->

    <owl:NamedIndividual rdf:about="http://purl.obolibrary.org/obo/GAZ_00326422">
        <rdf:type rdf:resource="http://purl.obolibrary.org/obo/ENVO_00000029"/>
        <obo:RO_0001025 rdf:resource="http://purl.obolibrary.org/obo/GAZ_00043994"/>
        <obo:IAO_0000115>A waterway.</obo:IAO_0000115>
        <oboInOwl:hasOBONamespace>GAZ</oboInOwl:hasOBONamespace>
        <oboInOwl:id>GAZ:00326422</oboInOwl:id>
        <rdfs:label>Wantij</rdfs:label>
    </owl:NamedIndividual>
    


    <!-- http://purl.obolibrary.org/obo/GAZ_00326432 -->

    <owl:NamedIndividual rdf:about="http://purl.obolibrary.org/obo/GAZ_00326432">
        <obo:IAO_0000115>A harbor.</obo:IAO_0000115>
        <oboInOwl:hasOBONamespace>GAZ</oboInOwl:hasOBONamespace>
        <oboInOwl:id>GAZ:00326432</oboInOwl:id>
        <rdfs:label>Zevenmanshaven</rdfs:label>
    </owl:NamedIndividual>
    


    <!-- http://purl.obolibrary.org/obo/GAZ_00326445 -->

    <owl:NamedIndividual rdf:about="http://purl.obolibrary.org/obo/GAZ_00326445">
        <obo:RO_0001025 rdf:resource="http://purl.obolibrary.org/obo/GAZ_00021319"/>
        <obo:IAO_0000115>A park.</obo:IAO_0000115>
        <oboInOwl:hasOBONamespace>GAZ</oboInOwl:hasOBONamespace>
        <oboInOwl:id>GAZ:00326445</oboInOwl:id>
        <rdfs:label>Donckse Bos</rdfs:label>
    </owl:NamedIndividual>
    


    <!-- http://purl.obolibrary.org/obo/GAZ_00326463 -->

    <owl:NamedIndividual rdf:about="http://purl.obolibrary.org/obo/GAZ_00326463">
        <obo:RO_0001025 rdf:resource="http://purl.obolibrary.org/obo/GAZ_00043988"/>
        <obo:IAO_0000115>A protected area.</obo:IAO_0000115>
        <oboInOwl:hasOBONamespace>GAZ</oboInOwl:hasOBONamespace>
        <oboInOwl:id>GAZ:00326463</oboInOwl:id>
        <rdfs:label>Kwade Hoek</rdfs:label>
    </owl:NamedIndividual>
    


    <!-- http://purl.obolibrary.org/obo/GAZ_00326465 -->

    <owl:NamedIndividual rdf:about="http://purl.obolibrary.org/obo/GAZ_00326465">
        <obo:RO_0001025 rdf:resource="http://purl.obolibrary.org/obo/GAZ_00021260"/>
        <obo:IAO_0000115>A protected area.</obo:IAO_0000115>
        <oboInOwl:hasOBONamespace>GAZ</oboInOwl:hasOBONamespace>
        <oboInOwl:id>GAZ:00326465</oboInOwl:id>
        <rdfs:label>Jan Gerritsepolder</rdfs:label>
    </owl:NamedIndividual>
    


    <!-- http://purl.obolibrary.org/obo/GAZ_00326476 -->

    <owl:NamedIndividual rdf:about="http://purl.obolibrary.org/obo/GAZ_00326476">
        <obo:RO_0001025 rdf:resource="http://purl.obolibrary.org/obo/GAZ_00144421"/>
        <obo:IAO_0000115>An island.</obo:IAO_0000115>
        <oboInOwl:hasOBONamespace>GAZ</oboInOwl:hasOBONamespace>
        <oboInOwl:id>GAZ:00326476</oboInOwl:id>
        <rdfs:label>Sophiapolder</rdfs:label>
    </owl:NamedIndividual>
    


    <!-- http://purl.obolibrary.org/obo/GAZ_00326491 -->

    <owl:NamedIndividual rdf:about="http://purl.obolibrary.org/obo/GAZ_00326491">
        <obo:RO_0001025 rdf:resource="http://purl.obolibrary.org/obo/GAZ_00043990"/>
        <obo:IAO_0000115>A river.</obo:IAO_0000115>
        <oboInOwl:hasOBONamespace>GAZ</oboInOwl:hasOBONamespace>
        <oboInOwl:id>GAZ:00326491</oboInOwl:id>
        <rdfs:label>Waaltje</rdfs:label>
    </owl:NamedIndividual>
    


    <!-- http://purl.obolibrary.org/obo/GAZ_00326516 -->

    <owl:NamedIndividual rdf:about="http://purl.obolibrary.org/obo/GAZ_00326516">
        <obo:RO_0001025 rdf:resource="http://purl.obolibrary.org/obo/GAZ_00144407"/>
        <obo:IAO_0000115>A harbor.</obo:IAO_0000115>
        <oboInOwl:hasOBONamespace>GAZ</oboInOwl:hasOBONamespace>
        <oboInOwl:id>GAZ:00326516</oboInOwl:id>
        <rdfs:label>Beneluxhaven</rdfs:label>
    </owl:NamedIndividual>
    


    <!-- http://purl.obolibrary.org/obo/GAZ_00326518 -->

    <owl:NamedIndividual rdf:about="http://purl.obolibrary.org/obo/GAZ_00326518">
        <obo:RO_0001025 rdf:resource="http://purl.obolibrary.org/obo/GAZ_00144407"/>
        <obo:IAO_0000115>A harbor.</obo:IAO_0000115>
        <oboInOwl:hasOBONamespace>GAZ</oboInOwl:hasOBONamespace>
        <oboInOwl:id>GAZ:00326518</oboInOwl:id>
        <rdfs:label>Brittanniehaven</rdfs:label>
    </owl:NamedIndividual>
    


    <!-- http://purl.obolibrary.org/obo/GAZ_00326519 -->

    <owl:NamedIndividual rdf:about="http://purl.obolibrary.org/obo/GAZ_00326519">
        <obo:RO_0001025 rdf:resource="http://purl.obolibrary.org/obo/GAZ_00144407"/>
        <obo:IAO_0000115>A harbor.</obo:IAO_0000115>
        <oboInOwl:hasOBONamespace>GAZ</oboInOwl:hasOBONamespace>
        <oboInOwl:id>GAZ:00326519</oboInOwl:id>
        <rdfs:label>Dintelhaven</rdfs:label>
    </owl:NamedIndividual>
    


    <!-- http://purl.obolibrary.org/obo/GAZ_00326531 -->

    <owl:NamedIndividual rdf:about="http://purl.obolibrary.org/obo/GAZ_00326531">
        <obo:RO_0001025 rdf:resource="http://purl.obolibrary.org/obo/GAZ_00144407"/>
        <obo:IAO_0000115>A harbor.</obo:IAO_0000115>
        <oboInOwl:hasOBONamespace>GAZ</oboInOwl:hasOBONamespace>
        <oboInOwl:id>GAZ:00326531</oboInOwl:id>
        <rdfs:label>Seinehaven</rdfs:label>
    </owl:NamedIndividual>
    


    <!-- http://purl.obolibrary.org/obo/GAZ_00326532 -->

    <owl:NamedIndividual rdf:about="http://purl.obolibrary.org/obo/GAZ_00326532">
        <obo:RO_0001025 rdf:resource="http://purl.obolibrary.org/obo/GAZ_00144407"/>
        <obo:IAO_0000115>A harbor.</obo:IAO_0000115>
        <oboInOwl:hasOBONamespace>GAZ</oboInOwl:hasOBONamespace>
        <oboInOwl:id>GAZ:00326532</oboInOwl:id>
        <rdfs:label>Neckarhaven</rdfs:label>
    </owl:NamedIndividual>
    


    <!-- http://purl.obolibrary.org/obo/GAZ_00326533 -->

    <owl:NamedIndividual rdf:about="http://purl.obolibrary.org/obo/GAZ_00326533">
        <obo:RO_0001025 rdf:resource="http://purl.obolibrary.org/obo/GAZ_00144407"/>
        <obo:IAO_0000115>A harbor.</obo:IAO_0000115>
        <oboInOwl:hasOBONamespace>GAZ</oboInOwl:hasOBONamespace>
        <oboInOwl:id>GAZ:00326533</oboInOwl:id>
        <rdfs:label>Londenhaven</rdfs:label>
    </owl:NamedIndividual>
    


    <!-- http://purl.obolibrary.org/obo/GAZ_00326534 -->

    <owl:NamedIndividual rdf:about="http://purl.obolibrary.org/obo/GAZ_00326534">
        <obo:RO_0001025 rdf:resource="http://purl.obolibrary.org/obo/GAZ_00144407"/>
        <obo:IAO_0000115>A harbor.</obo:IAO_0000115>
        <oboInOwl:hasOBONamespace>GAZ</oboInOwl:hasOBONamespace>
        <oboInOwl:id>GAZ:00326534</oboInOwl:id>
        <rdfs:label>Zevende Petroleumhaven</rdfs:label>
    </owl:NamedIndividual>
    


    <!-- http://purl.obolibrary.org/obo/GAZ_00326535 -->

    <owl:NamedIndividual rdf:about="http://purl.obolibrary.org/obo/GAZ_00326535">
        <obo:RO_0001025 rdf:resource="http://purl.obolibrary.org/obo/GAZ_00144407"/>
        <obo:IAO_0000115>A harbor.</obo:IAO_0000115>
        <oboInOwl:hasOBONamespace>GAZ</oboInOwl:hasOBONamespace>
        <oboInOwl:id>GAZ:00326535</oboInOwl:id>
        <rdfs:label>Donauhaven</rdfs:label>
    </owl:NamedIndividual>
    


    <!-- http://purl.obolibrary.org/obo/GAZ_00326536 -->

    <owl:NamedIndividual rdf:about="http://purl.obolibrary.org/obo/GAZ_00326536">
        <obo:RO_0001025 rdf:resource="http://purl.obolibrary.org/obo/GAZ_00144407"/>
        <obo:IAO_0000115>A harbor.</obo:IAO_0000115>
        <oboInOwl:hasOBONamespace>GAZ</oboInOwl:hasOBONamespace>
        <oboInOwl:id>GAZ:00326536</oboInOwl:id>
        <rdfs:label>Wezerhaven</rdfs:label>
    </owl:NamedIndividual>
    


    <!-- http://purl.obolibrary.org/obo/GAZ_00326537 -->

    <owl:NamedIndividual rdf:about="http://purl.obolibrary.org/obo/GAZ_00326537">
        <obo:RO_0001025 rdf:resource="http://purl.obolibrary.org/obo/GAZ_00144407"/>
        <obo:IAO_0000115>A harbor.</obo:IAO_0000115>
        <oboInOwl:hasOBONamespace>GAZ</oboInOwl:hasOBONamespace>
        <oboInOwl:id>GAZ:00326537</oboInOwl:id>
        <rdfs:label>Vijfde Petroleumhaven</rdfs:label>
    </owl:NamedIndividual>
    


    <!-- http://purl.obolibrary.org/obo/GAZ_00326538 -->

    <owl:NamedIndividual rdf:about="http://purl.obolibrary.org/obo/GAZ_00326538">
        <obo:RO_0001025 rdf:resource="http://purl.obolibrary.org/obo/GAZ_00144407"/>
        <obo:IAO_0000115>A harbor.</obo:IAO_0000115>
        <oboInOwl:hasOBONamespace>GAZ</oboInOwl:hasOBONamespace>
        <oboInOwl:id>GAZ:00326538</oboInOwl:id>
        <rdfs:label>Vierde Petroleumhaven</rdfs:label>
    </owl:NamedIndividual>
    


    <!-- http://purl.obolibrary.org/obo/GAZ_00326539 -->

    <owl:NamedIndividual rdf:about="http://purl.obolibrary.org/obo/GAZ_00326539">
        <obo:RO_0001025 rdf:resource="http://purl.obolibrary.org/obo/GAZ_00144407"/>
        <obo:IAO_0000115>A harbor.</obo:IAO_0000115>
        <oboInOwl:hasOBONamespace>GAZ</oboInOwl:hasOBONamespace>
        <oboInOwl:id>GAZ:00326539</oboInOwl:id>
        <rdfs:label>Scheurhaven</rdfs:label>
    </owl:NamedIndividual>
    


    <!-- http://purl.obolibrary.org/obo/GAZ_00326540 -->

    <owl:NamedIndividual rdf:about="http://purl.obolibrary.org/obo/GAZ_00326540">
        <obo:RO_0001025 rdf:resource="http://purl.obolibrary.org/obo/GAZ_00144407"/>
        <obo:IAO_0000115>A harbor.</obo:IAO_0000115>
        <oboInOwl:hasOBONamespace>GAZ</oboInOwl:hasOBONamespace>
        <oboInOwl:id>GAZ:00326540</oboInOwl:id>
        <rdfs:label>Elbehaven</rdfs:label>
    </owl:NamedIndividual>
    


    <!-- http://purl.obolibrary.org/obo/GAZ_00326541 -->

    <owl:NamedIndividual rdf:about="http://purl.obolibrary.org/obo/GAZ_00326541">
        <obo:RO_0001025 rdf:resource="http://purl.obolibrary.org/obo/GAZ_00144407"/>
        <obo:IAO_0000115>A harbor.</obo:IAO_0000115>
        <oboInOwl:hasOBONamespace>GAZ</oboInOwl:hasOBONamespace>
        <oboInOwl:id>GAZ:00326541</oboInOwl:id>
        <rdfs:label>Dommelhaven</rdfs:label>
    </owl:NamedIndividual>
    


    <!-- http://purl.obolibrary.org/obo/GAZ_00326559 -->

    <owl:NamedIndividual rdf:about="http://purl.obolibrary.org/obo/GAZ_00326559">
        <obo:IAO_0000115>A Canal.</obo:IAO_0000115>
        <oboInOwl:hasOBONamespace>GAZ</oboInOwl:hasOBONamespace>
        <oboInOwl:id>GAZ:00326559</oboInOwl:id>
        <rdfs:label>Woudwetering</rdfs:label>
    </owl:NamedIndividual>
    


    <!-- http://purl.obolibrary.org/obo/GAZ_00326631 -->

    <owl:NamedIndividual rdf:about="http://purl.obolibrary.org/obo/GAZ_00326631">
        <obo:RO_0001025 rdf:resource="http://purl.obolibrary.org/obo/GAZ_00325986"/>
        <obo:IAO_0000115>A protected area.</obo:IAO_0000115>
        <oboInOwl:hasOBONamespace>GAZ</oboInOwl:hasOBONamespace>
        <oboInOwl:id>GAZ:00326631</oboInOwl:id>
        <rdfs:label>Bloemdijken van Zuid-Beveland</rdfs:label>
    </owl:NamedIndividual>
    


    <!-- http://purl.obolibrary.org/obo/GAZ_00326634 -->

    <owl:NamedIndividual rdf:about="http://purl.obolibrary.org/obo/GAZ_00326634">
        <obo:RO_0001025 rdf:resource="http://purl.obolibrary.org/obo/GAZ_00144361"/>
        <obo:IAO_0000115>A protected area.</obo:IAO_0000115>
        <oboInOwl:hasOBONamespace>GAZ</oboInOwl:hasOBONamespace>
        <oboInOwl:id>GAZ:00326634</oboInOwl:id>
        <rdfs:label>De Plate</rdfs:label>
    </owl:NamedIndividual>
    


    <!-- http://purl.obolibrary.org/obo/GAZ_00326638 -->

    <owl:NamedIndividual rdf:about="http://purl.obolibrary.org/obo/GAZ_00326638">
        <obo:RO_0001025 rdf:resource="http://purl.obolibrary.org/obo/GAZ_00021224"/>
        <obo:IAO_0000115>A dune system.</obo:IAO_0000115>
        <oboInOwl:hasOBONamespace>GAZ</oboInOwl:hasOBONamespace>
        <oboInOwl:id>GAZ:00326638</oboInOwl:id>
        <rdfs:label>Kaloot</rdfs:label>
    </owl:NamedIndividual>
    


    <!-- http://purl.obolibrary.org/obo/GAZ_00326639 -->

    <owl:NamedIndividual rdf:about="http://purl.obolibrary.org/obo/GAZ_00326639">
        <obo:RO_0001025 rdf:resource="http://purl.obolibrary.org/obo/GAZ_00012545"/>
        <obo:IAO_0000115>A protected area.</obo:IAO_0000115>
        <oboInOwl:hasOBONamespace>GAZ</oboInOwl:hasOBONamespace>
        <oboInOwl:id>GAZ:00326639</oboInOwl:id>
        <rdfs:label>Oosterschenge</rdfs:label>
    </owl:NamedIndividual>
    


    <!-- http://purl.obolibrary.org/obo/GAZ_00326640 -->

    <owl:NamedIndividual rdf:about="http://purl.obolibrary.org/obo/GAZ_00326640">
        <obo:RO_0001025 rdf:resource="http://purl.obolibrary.org/obo/GAZ_00021229"/>
        <obo:IAO_0000115>A populated place.</obo:IAO_0000115>
        <oboInOwl:hasOBONamespace>GAZ</oboInOwl:hasOBONamespace>
        <oboInOwl:id>GAZ:00326640</oboInOwl:id>
        <rdfs:label>Serooskerke</rdfs:label>
    </owl:NamedIndividual>
    


    <!-- http://purl.obolibrary.org/obo/GAZ_00326641 -->

    <owl:NamedIndividual rdf:about="http://purl.obolibrary.org/obo/GAZ_00326641">
        <obo:RO_0001025 rdf:resource="http://purl.obolibrary.org/obo/GAZ_00326640"/>
        <obo:IAO_0000115>A protected area.</obo:IAO_0000115>
        <oboInOwl:hasOBONamespace>GAZ</oboInOwl:hasOBONamespace>
        <oboInOwl:id>GAZ:00326641</oboInOwl:id>
        <rdfs:label>Schelphoek</rdfs:label>
    </owl:NamedIndividual>
    


    <!-- http://purl.obolibrary.org/obo/GAZ_00326643 -->

    <owl:NamedIndividual rdf:about="http://purl.obolibrary.org/obo/GAZ_00326643">
        <obo:RO_0001025 rdf:resource="http://purl.obolibrary.org/obo/GAZ_00144361"/>
        <obo:IAO_0000115>A brackish wetland. A protected area.</obo:IAO_0000115>
        <oboInOwl:hasOBONamespace>GAZ</oboInOwl:hasOBONamespace>
        <oboInOwl:id>GAZ:00326643</oboInOwl:id>
        <rdfs:label>Verdronken Land van Saeftinghe</rdfs:label>
    </owl:NamedIndividual>
    


    <!-- http://purl.obolibrary.org/obo/GAZ_00326644 -->

    <owl:NamedIndividual rdf:about="http://purl.obolibrary.org/obo/GAZ_00326644">
        <obo:RO_0001025 rdf:resource="http://purl.obolibrary.org/obo/GAZ_00090210"/>
        <obo:IAO_0000115>A protected area.</obo:IAO_0000115>
        <oboInOwl:hasOBONamespace>GAZ</oboInOwl:hasOBONamespace>
        <oboInOwl:id>GAZ:00326644</oboInOwl:id>
        <rdfs:label>Verdronken Land van Zuid-Beveland</rdfs:label>
    </owl:NamedIndividual>
    


    <!-- http://purl.obolibrary.org/obo/GAZ_00326647 -->

    <owl:NamedIndividual rdf:about="http://purl.obolibrary.org/obo/GAZ_00326647">
        <obo:RO_0001025 rdf:resource="http://purl.obolibrary.org/obo/GAZ_00021224"/>
        <obo:IAO_0000115>A protected area.</obo:IAO_0000115>
        <oboInOwl:hasOBONamespace>GAZ</oboInOwl:hasOBONamespace>
        <oboInOwl:id>GAZ:00326647</oboInOwl:id>
        <rdfs:label>Westeindse Weel</rdfs:label>
    </owl:NamedIndividual>
    


    <!-- http://purl.obolibrary.org/obo/GAZ_00326648 -->

    <owl:NamedIndividual rdf:about="http://purl.obolibrary.org/obo/GAZ_00326648">
        <obo:RO_0001025 rdf:resource="http://purl.obolibrary.org/obo/GAZ_00012545"/>
        <obo:IAO_0000115>A protected area.</obo:IAO_0000115>
        <oboInOwl:hasOBONamespace>GAZ</oboInOwl:hasOBONamespace>
        <oboInOwl:id>GAZ:00326648</oboInOwl:id>
        <rdfs:label>Westerschenge</rdfs:label>
    </owl:NamedIndividual>
    


    <!-- http://purl.obolibrary.org/obo/GAZ_00326649 -->

    <owl:NamedIndividual rdf:about="http://purl.obolibrary.org/obo/GAZ_00326649">
        <obo:RO_0001025 rdf:resource="http://purl.obolibrary.org/obo/GAZ_00144362"/>
        <obo:IAO_0000115>A protected area.</obo:IAO_0000115>
        <oboInOwl:hasOBONamespace>GAZ</oboInOwl:hasOBONamespace>
        <oboInOwl:id>GAZ:00326649</oboInOwl:id>
        <rdfs:label>Yerseke Moer</rdfs:label>
    </owl:NamedIndividual>
    


    <!-- http://purl.obolibrary.org/obo/GAZ_00326650 -->

    <owl:NamedIndividual rdf:about="http://purl.obolibrary.org/obo/GAZ_00326650">
        <obo:RO_0001025 rdf:resource="http://purl.obolibrary.org/obo/GAZ_00021224"/>
        <obo:IAO_0000115>A populated place.</obo:IAO_0000115>
        <oboInOwl:hasOBONamespace>GAZ</oboInOwl:hasOBONamespace>
        <oboInOwl:id>GAZ:00326650</oboInOwl:id>
        <rdfs:label>Kwadendamme</rdfs:label>
    </owl:NamedIndividual>
    


    <!-- http://purl.obolibrary.org/obo/GAZ_00326651 -->

    <owl:NamedIndividual rdf:about="http://purl.obolibrary.org/obo/GAZ_00326651">
        <obo:RO_0001025 rdf:resource="http://purl.obolibrary.org/obo/GAZ_00326650"/>
        <obo:IAO_0000115>A protected area. A wetland.</obo:IAO_0000115>
        <oboInOwl:hasOBONamespace>GAZ</oboInOwl:hasOBONamespace>
        <oboInOwl:id>GAZ:00326651</oboInOwl:id>
        <rdfs:label>Zwaakse Weel</rdfs:label>
    </owl:NamedIndividual>
    


    <!-- http://purl.obolibrary.org/obo/GAZ_00326658 -->

    <owl:NamedIndividual rdf:about="http://purl.obolibrary.org/obo/GAZ_00326658">
        <obo:RO_0001025 rdf:resource="http://purl.obolibrary.org/obo/GAZ_00005544"/>
        <obo:IAO_0000115>A populated place.</obo:IAO_0000115>
        <oboInOwl:hasOBONamespace>GAZ</oboInOwl:hasOBONamespace>
        <oboInOwl:id>GAZ:00326658</oboInOwl:id>
        <rdfs:label>Goese Sas</rdfs:label>
    </owl:NamedIndividual>
    


    <!-- http://purl.obolibrary.org/obo/GAZ_00326661 -->

    <owl:NamedIndividual rdf:about="http://purl.obolibrary.org/obo/GAZ_00326661">
        <obo:RO_0001025 rdf:resource="http://purl.obolibrary.org/obo/GAZ_00144361"/>
        <obo:IAO_0000115>A river.</obo:IAO_0000115>
        <oboInOwl:hasOBONamespace>GAZ</oboInOwl:hasOBONamespace>
        <oboInOwl:id>GAZ:00326661</oboInOwl:id>
        <rdfs:label>Honte</rdfs:label>
    </owl:NamedIndividual>
    


    <!-- http://purl.obolibrary.org/obo/GAZ_00326666 -->

    <owl:NamedIndividual rdf:about="http://purl.obolibrary.org/obo/GAZ_00326666">
        <obo:RO_0001025 rdf:resource="http://purl.obolibrary.org/obo/GAZ_00144371"/>
        <obo:IAO_0000115>A channel.</obo:IAO_0000115>
        <oboInOwl:hasOBONamespace>GAZ</oboInOwl:hasOBONamespace>
        <oboInOwl:id>GAZ:00326666</oboInOwl:id>
        <rdfs:label>Oostgat</rdfs:label>
    </owl:NamedIndividual>
    


    <!-- http://purl.obolibrary.org/obo/GAZ_00326668 -->

    <owl:NamedIndividual rdf:about="http://purl.obolibrary.org/obo/GAZ_00326668">
        <obo:RO_0001025 rdf:resource="http://purl.obolibrary.org/obo/GAZ_00144373"/>
        <obo:IAO_0000115>A channel.</obo:IAO_0000115>
        <oboInOwl:hasOBONamespace>GAZ</oboInOwl:hasOBONamespace>
        <oboInOwl:id>GAZ:00326668</oboInOwl:id>
        <rdfs:label>Roompot</rdfs:label>
    </owl:NamedIndividual>
    


    <!-- http://purl.obolibrary.org/obo/GAZ_00326673 -->

    <owl:NamedIndividual rdf:about="http://purl.obolibrary.org/obo/GAZ_00326673">
        <obo:RO_0001025 rdf:resource="http://purl.obolibrary.org/obo/GAZ_00144361"/>
        <obo:IAO_0000115>A channel.</obo:IAO_0000115>
        <oboInOwl:hasOBONamespace>GAZ</oboInOwl:hasOBONamespace>
        <oboInOwl:id>GAZ:00326673</oboInOwl:id>
        <rdfs:label>Wielingen</rdfs:label>
    </owl:NamedIndividual>
    


    <!-- http://purl.obolibrary.org/obo/GAZ_00326675 -->

    <owl:NamedIndividual rdf:about="http://purl.obolibrary.org/obo/GAZ_00326675">
        <obo:RO_0001025 rdf:resource="http://purl.obolibrary.org/obo/GAZ_00144362"/>
        <obo:IAO_0000115>A lake.</obo:IAO_0000115>
        <oboInOwl:hasOBONamespace>GAZ</oboInOwl:hasOBONamespace>
        <oboInOwl:id>GAZ:00326675</oboInOwl:id>
        <rdfs:label>Zoommeer</rdfs:label>
    </owl:NamedIndividual>
    


    <!-- http://purl.obolibrary.org/obo/GAZ_00326715 -->

    <owl:NamedIndividual rdf:about="http://purl.obolibrary.org/obo/GAZ_00326715">
        <obo:RO_0001025 rdf:resource="http://purl.obolibrary.org/obo/GAZ_00144423"/>
        <obo:IAO_0000115>A man-made island.</obo:IAO_0000115>
        <oboInOwl:hasOBONamespace>GAZ</oboInOwl:hasOBONamespace>
        <oboInOwl:id>GAZ:00326715</oboInOwl:id>
        <rdfs:label>Neeltje Jans</rdfs:label>
    </owl:NamedIndividual>
    


    <!-- http://purl.obolibrary.org/obo/GAZ_00326716 -->

    <owl:NamedIndividual rdf:about="http://purl.obolibrary.org/obo/GAZ_00326716">
        <obo:RO_0001025 rdf:resource="http://purl.obolibrary.org/obo/GAZ_00043996"/>
        <obo:IAO_0000115>A former island.</obo:IAO_0000115>
        <oboInOwl:hasOBONamespace>GAZ</oboInOwl:hasOBONamespace>
        <oboInOwl:id>GAZ:00326716</oboInOwl:id>
        <rdfs:label>Bommenede</rdfs:label>
    </owl:NamedIndividual>
    


    <!-- http://purl.obolibrary.org/obo/GAZ_00326717 -->

    <owl:NamedIndividual rdf:about="http://purl.obolibrary.org/obo/GAZ_00326717">
        <obo:RO_0001025 rdf:resource="http://purl.obolibrary.org/obo/GAZ_00043996"/>
        <obo:IAO_0000115>A former island.</obo:IAO_0000115>
        <oboInOwl:hasOBONamespace>GAZ</oboInOwl:hasOBONamespace>
        <oboInOwl:id>GAZ:00326717</oboInOwl:id>
        <rdfs:label>Duiveland</rdfs:label>
    </owl:NamedIndividual>
    


    <!-- http://purl.obolibrary.org/obo/GAZ_00326718 -->

    <owl:NamedIndividual rdf:about="http://purl.obolibrary.org/obo/GAZ_00326718">
        <obo:RO_0001025 rdf:resource="http://purl.obolibrary.org/obo/GAZ_00326661"/>
        <obo:IAO_0000115>A former island. Destroyed by floods 1570.</obo:IAO_0000115>
        <oboInOwl:hasOBONamespace>GAZ</oboInOwl:hasOBONamespace>
        <oboInOwl:id>GAZ:00326718</oboInOwl:id>
        <rdfs:label>Koezand</rdfs:label>
    </owl:NamedIndividual>
    


    <!-- http://purl.obolibrary.org/obo/GAZ_00326719 -->

    <owl:NamedIndividual rdf:about="http://purl.obolibrary.org/obo/GAZ_00326719">
        <obo:RO_0001025 rdf:resource="http://purl.obolibrary.org/obo/GAZ_00090210"/>
        <obo:IAO_0000115>A former island.</obo:IAO_0000115>
        <oboInOwl:hasOBONamespace>GAZ</oboInOwl:hasOBONamespace>
        <oboInOwl:id>GAZ:00326719</oboInOwl:id>
        <rdfs:label>Orisant</rdfs:label>
    </owl:NamedIndividual>
    


    <!-- http://purl.obolibrary.org/obo/GAZ_00326720 -->

    <owl:NamedIndividual rdf:about="http://purl.obolibrary.org/obo/GAZ_00326720">
        <obo:RO_0001025 rdf:resource="http://purl.obolibrary.org/obo/GAZ_00043996"/>
        <obo:IAO_0000115>A former island.</obo:IAO_0000115>
        <oboInOwl:hasOBONamespace>GAZ</oboInOwl:hasOBONamespace>
        <oboInOwl:id>GAZ:00326720</oboInOwl:id>
        <rdfs:label>Schouwen</rdfs:label>
    </owl:NamedIndividual>
    


    <!-- http://purl.obolibrary.org/obo/GAZ_00326721 -->

    <owl:NamedIndividual rdf:about="http://purl.obolibrary.org/obo/GAZ_00326721">
        <obo:RO_0001025 rdf:resource="http://purl.obolibrary.org/obo/GAZ_00021224"/>
        <obo:IAO_0000115>A populated place.</obo:IAO_0000115>
        <oboInOwl:hasOBONamespace>GAZ</oboInOwl:hasOBONamespace>
        <oboInOwl:id>GAZ:00326721</oboInOwl:id>
        <rdfs:label>Baarland</rdfs:label>
    </owl:NamedIndividual>
    


    <!-- http://purl.obolibrary.org/obo/GAZ_00326722 -->

    <owl:NamedIndividual rdf:about="http://purl.obolibrary.org/obo/GAZ_00326722">
        <obo:RO_0001025 rdf:resource="http://purl.obolibrary.org/obo/GAZ_00326721"/>
        <obo:IAO_0000115>A former island.</obo:IAO_0000115>
        <oboInOwl:hasOBONamespace>GAZ</oboInOwl:hasOBONamespace>
        <oboInOwl:id>GAZ:00326722</oboInOwl:id>
        <rdfs:label>Stuivezand</rdfs:label>
    </owl:NamedIndividual>
    


    <!-- http://purl.obolibrary.org/obo/GAZ_00326723 -->

    <owl:NamedIndividual rdf:about="http://purl.obolibrary.org/obo/GAZ_00326723">
        <obo:RO_0001025 rdf:resource="http://purl.obolibrary.org/obo/GAZ_00144361"/>
        <obo:IAO_0000115>A former island.</obo:IAO_0000115>
        <oboInOwl:hasOBONamespace>GAZ</oboInOwl:hasOBONamespace>
        <oboInOwl:id>GAZ:00326723</oboInOwl:id>
        <rdfs:label>Waterdunen</rdfs:label>
    </owl:NamedIndividual>
    


    <!-- http://purl.obolibrary.org/obo/GAZ_00326724 -->

    <owl:NamedIndividual rdf:about="http://purl.obolibrary.org/obo/GAZ_00326724">
        <obo:RO_0001025 rdf:resource="http://purl.obolibrary.org/obo/GAZ_00144361"/>
        <obo:IAO_0000115>A former island.</obo:IAO_0000115>
        <oboInOwl:hasOBONamespace>GAZ</oboInOwl:hasOBONamespace>
        <oboInOwl:id>GAZ:00326724</oboInOwl:id>
        <rdfs:label>Wulpen</rdfs:label>
    </owl:NamedIndividual>
    


    <!-- http://purl.obolibrary.org/obo/GAZ_00326725 -->

    <owl:NamedIndividual rdf:about="http://purl.obolibrary.org/obo/GAZ_00326725">
        <obo:RO_0001025 rdf:resource="http://purl.obolibrary.org/obo/GAZ_00144392"/>
        <obo:IAO_0000115>An island.</obo:IAO_0000115>
        <oboInOwl:hasOBONamespace>GAZ</oboInOwl:hasOBONamespace>
        <oboInOwl:id>GAZ:00326725</oboInOwl:id>
        <rdfs:label>Eiland van Brienenoord</rdfs:label>
    </owl:NamedIndividual>
    


    <!-- http://purl.obolibrary.org/obo/GAZ_00326726 -->

    <owl:NamedIndividual rdf:about="http://purl.obolibrary.org/obo/GAZ_00326726">
        <obo:RO_0001025 rdf:resource="http://purl.obolibrary.org/obo/GAZ_00144392"/>
        <obo:IAO_0000115>An island.</obo:IAO_0000115>
        <oboInOwl:hasOBONamespace>GAZ</oboInOwl:hasOBONamespace>
        <oboInOwl:id>GAZ:00326726</oboInOwl:id>
        <rdfs:label>Noordereiland</rdfs:label>
    </owl:NamedIndividual>
    


    <!-- http://purl.obolibrary.org/obo/GAZ_00326730 -->

    <owl:NamedIndividual rdf:about="http://purl.obolibrary.org/obo/GAZ_00326730">
        <obo:IAO_0000115>A dam.</obo:IAO_0000115>
        <oboInOwl:hasOBONamespace>GAZ</oboInOwl:hasOBONamespace>
        <oboInOwl:id>GAZ:00326730</oboInOwl:id>
        <rdfs:label>Philipsdam</rdfs:label>
    </owl:NamedIndividual>
    


    <!-- http://purl.obolibrary.org/obo/GAZ_00326731 -->

    <owl:NamedIndividual rdf:about="http://purl.obolibrary.org/obo/GAZ_00326731">
        <obo:RO_0001025 rdf:resource="http://purl.obolibrary.org/obo/GAZ_00043988"/>
        <obo:IAO_0000115>A former island.</obo:IAO_0000115>
        <oboInOwl:hasOBONamespace>GAZ</oboInOwl:hasOBONamespace>
        <oboInOwl:id>GAZ:00326731</oboInOwl:id>
        <rdfs:label>Overflakkee</rdfs:label>
    </owl:NamedIndividual>
    


    <!-- http://purl.obolibrary.org/obo/GAZ_00326814 -->

    <owl:NamedIndividual rdf:about="http://purl.obolibrary.org/obo/GAZ_00326814">
        <obo:RO_0001025 rdf:resource="http://purl.obolibrary.org/obo/GAZ_00012576"/>
        <obo:IAO_0000115>A protected area.</obo:IAO_0000115>
        <oboInOwl:hasOBONamespace>GAZ</oboInOwl:hasOBONamespace>
        <oboInOwl:id>GAZ:00326814</oboInOwl:id>
        <rdfs:label>Manteling van Walcheren</rdfs:label>
    </owl:NamedIndividual>
    


    <!-- http://purl.obolibrary.org/obo/GAZ_00326818 -->

    <owl:NamedIndividual rdf:about="http://purl.obolibrary.org/obo/GAZ_00326818">
        <obo:RO_0001025 rdf:resource="http://purl.obolibrary.org/obo/GAZ_00021272"/>
        <obo:IAO_0000115>A protected area.</obo:IAO_0000115>
        <oboInOwl:hasOBONamespace>GAZ</oboInOwl:hasOBONamespace>
        <oboInOwl:id>GAZ:00326818</oboInOwl:id>
        <rdfs:label>Duinen Goeree &amp; Kwade Hoek</rdfs:label>
    </owl:NamedIndividual>
    


    <!-- http://purl.obolibrary.org/obo/GAZ_00343732 -->

    <owl:NamedIndividual rdf:about="http://purl.obolibrary.org/obo/GAZ_00343732">
        <obo:IAO_0000115>A canal.</obo:IAO_0000115>
        <oboInOwl:hasOBONamespace>GAZ</oboInOwl:hasOBONamespace>
        <oboInOwl:id>GAZ:00343732</oboInOwl:id>
        <rdfs:label>Canal de la Bruche</rdfs:label>
    </owl:NamedIndividual>
    


    <!-- http://purl.obolibrary.org/obo/GAZ_00343850 -->

    <owl:NamedIndividual rdf:about="http://purl.obolibrary.org/obo/GAZ_00343850">
        <obo:IAO_0000115>A river.</obo:IAO_0000115>
        <oboInOwl:hasOBONamespace>GAZ</oboInOwl:hasOBONamespace>
        <oboInOwl:id>GAZ:00343850</oboInOwl:id>
        <rdfs:label>Doller</rdfs:label>
    </owl:NamedIndividual>
    


    <!-- http://purl.obolibrary.org/obo/GAZ_00343963 -->

    <owl:NamedIndividual rdf:about="http://purl.obolibrary.org/obo/GAZ_00343963">
        <obo:IAO_0000115>A river.</obo:IAO_0000115>
        <oboInOwl:hasOBONamespace>GAZ</oboInOwl:hasOBONamespace>
        <oboInOwl:id>GAZ:00343963</oboInOwl:id>
        <rdfs:label>Blind</rdfs:label>
    </owl:NamedIndividual>
    


    <!-- http://purl.obolibrary.org/obo/GAZ_00343973 -->

    <owl:NamedIndividual rdf:about="http://purl.obolibrary.org/obo/GAZ_00343973">
        <obo:IAO_0000115>A river.</obo:IAO_0000115>
        <oboInOwl:hasOBONamespace>GAZ</oboInOwl:hasOBONamespace>
        <oboInOwl:id>GAZ:00343973</oboInOwl:id>
        <rdfs:label>Erlenbach</rdfs:label>
    </owl:NamedIndividual>
    


    <!-- http://purl.obolibrary.org/obo/GAZ_00344016 -->

    <owl:NamedIndividual rdf:about="http://purl.obolibrary.org/obo/GAZ_00344016">
        <obo:IAO_0000115>The historic centre of Strasbourg, France, is an island in the Ill River.</obo:IAO_0000115>
        <oboInOwl:hasOBONamespace>GAZ</oboInOwl:hasOBONamespace>
        <oboInOwl:id>GAZ:00344016</oboInOwl:id>
        <rdfs:label>Grande Ile de Strasbourg</rdfs:label>
    </owl:NamedIndividual>
    


    <!-- http://purl.obolibrary.org/obo/GAZ_00344017 -->

    <owl:NamedIndividual rdf:about="http://purl.obolibrary.org/obo/GAZ_00344017">
        <obo:RO_0001025 rdf:resource="http://purl.obolibrary.org/obo/GAZ_00008262"/>
        <obo:IAO_0000115>An island.</obo:IAO_0000115>
        <oboInOwl:hasOBONamespace>GAZ</oboInOwl:hasOBONamespace>
        <oboInOwl:id>GAZ:00344017</oboInOwl:id>
        <rdfs:label>Ile aux Epis</rdfs:label>
    </owl:NamedIndividual>
    


    <!-- http://purl.obolibrary.org/obo/GAZ_00344019 -->

    <owl:NamedIndividual rdf:about="http://purl.obolibrary.org/obo/GAZ_00344019">
        <obo:RO_0001025 rdf:resource="http://purl.obolibrary.org/obo/GAZ_00344016"/>
        <obo:IAO_0000115>A quartier of Strasbourg.</obo:IAO_0000115>
        <oboInOwl:hasOBONamespace>GAZ</oboInOwl:hasOBONamespace>
        <oboInOwl:id>GAZ:00344019</oboInOwl:id>
        <rdfs:label>Centre</rdfs:label>
    </owl:NamedIndividual>
    


    <!-- http://purl.obolibrary.org/obo/GAZ_00344140 -->

    <owl:NamedIndividual rdf:about="http://purl.obolibrary.org/obo/GAZ_00344140">
        <obo:IAO_0000115>A river.</obo:IAO_0000115>
        <oboInOwl:hasOBONamespace>GAZ</oboInOwl:hasOBONamespace>
        <oboInOwl:id>GAZ:00344140</oboInOwl:id>
        <rdfs:label>Ruisseau du lac Noir</rdfs:label>
    </owl:NamedIndividual>
    


    <!-- http://purl.obolibrary.org/obo/GAZ_00344141 -->

    <owl:NamedIndividual rdf:about="http://purl.obolibrary.org/obo/GAZ_00344141">
        <obo:IAO_0000115>A river.</obo:IAO_0000115>
        <oboInOwl:hasOBONamespace>GAZ</oboInOwl:hasOBONamespace>
        <oboInOwl:id>GAZ:00344141</oboInOwl:id>
        <rdfs:label>Ruisseau du Lac Blanc</rdfs:label>
    </owl:NamedIndividual>
    


    <!-- http://purl.obolibrary.org/obo/GAZ_00344142 -->

    <owl:NamedIndividual rdf:about="http://purl.obolibrary.org/obo/GAZ_00344142">
        <obo:IAO_0000115>A river.</obo:IAO_0000115>
        <oboInOwl:hasOBONamespace>GAZ</oboInOwl:hasOBONamespace>
        <oboInOwl:id>GAZ:00344142</oboInOwl:id>
        <rdfs:label>Ruisseau le Surcenord</rdfs:label>
    </owl:NamedIndividual>
    


    <!-- http://purl.obolibrary.org/obo/GAZ_00344416 -->

    <owl:NamedIndividual rdf:about="http://purl.obolibrary.org/obo/GAZ_00344416">
        <obo:IAO_0000115>A river.</obo:IAO_0000115>
        <oboInOwl:hasOBONamespace>GAZ</oboInOwl:hasOBONamespace>
        <oboInOwl:id>GAZ:00344416</oboInOwl:id>
        <rdfs:label>Lawinenrunz</rdfs:label>
    </owl:NamedIndividual>
    


    <!-- http://purl.obolibrary.org/obo/GAZ_00344417 -->

    <owl:NamedIndividual rdf:about="http://purl.obolibrary.org/obo/GAZ_00344417">
        <obo:IAO_0000115>A river.</obo:IAO_0000115>
        <oboInOwl:hasOBONamespace>GAZ</oboInOwl:hasOBONamespace>
        <oboInOwl:id>GAZ:00344417</oboInOwl:id>
        <rdfs:label>Ruisseau de l&apos;Hinter Bockloch</rdfs:label>
    </owl:NamedIndividual>
    


    <!-- http://purl.obolibrary.org/obo/GAZ_00344418 -->

    <owl:NamedIndividual rdf:about="http://purl.obolibrary.org/obo/GAZ_00344418">
        <obo:IAO_0000115>A river.</obo:IAO_0000115>
        <oboInOwl:hasOBONamespace>GAZ</oboInOwl:hasOBONamespace>
        <oboInOwl:id>GAZ:00344418</oboInOwl:id>
        <rdfs:label>Ruisseau du Vorder Bockloch</rdfs:label>
    </owl:NamedIndividual>
    


    <!-- http://purl.obolibrary.org/obo/GAZ_00344419 -->

    <owl:NamedIndividual rdf:about="http://purl.obolibrary.org/obo/GAZ_00344419">
        <obo:IAO_0000115>A river.</obo:IAO_0000115>
        <oboInOwl:hasOBONamespace>GAZ</oboInOwl:hasOBONamespace>
        <oboInOwl:id>GAZ:00344419</oboInOwl:id>
        <rdfs:label>Tieferunz</rdfs:label>
    </owl:NamedIndividual>
    


    <!-- http://purl.obolibrary.org/obo/GAZ_00344422 -->

    <owl:NamedIndividual rdf:about="http://purl.obolibrary.org/obo/GAZ_00344422">
        <obo:IAO_0000115>A river.</obo:IAO_0000115>
        <oboInOwl:hasOBONamespace>GAZ</oboInOwl:hasOBONamespace>
        <oboInOwl:id>GAZ:00344422</oboInOwl:id>
        <rdfs:label>Runscherunz</rdfs:label>
    </owl:NamedIndividual>
    


    <!-- http://purl.obolibrary.org/obo/GAZ_00344426 -->

    <owl:NamedIndividual rdf:about="http://purl.obolibrary.org/obo/GAZ_00344426">
        <obo:IAO_0000115>A river.</obo:IAO_0000115>
        <oboInOwl:hasOBONamespace>GAZ</oboInOwl:hasOBONamespace>
        <oboInOwl:id>GAZ:00344426</oboInOwl:id>
        <rdfs:label>Gottrunz</rdfs:label>
    </owl:NamedIndividual>
    


    <!-- http://purl.obolibrary.org/obo/GAZ_00344428 -->

    <owl:NamedIndividual rdf:about="http://purl.obolibrary.org/obo/GAZ_00344428">
        <obo:IAO_0000115>A river.</obo:IAO_0000115>
        <oboInOwl:hasOBONamespace>GAZ</oboInOwl:hasOBONamespace>
        <oboInOwl:id>GAZ:00344428</oboInOwl:id>
        <rdfs:label>Rammersbach</rdfs:label>
    </owl:NamedIndividual>
    


    <!-- http://purl.obolibrary.org/obo/GAZ_00344430 -->

    <owl:NamedIndividual rdf:about="http://purl.obolibrary.org/obo/GAZ_00344430">
        <obo:IAO_0000115>A river.</obo:IAO_0000115>
        <oboInOwl:hasOBONamespace>GAZ</oboInOwl:hasOBONamespace>
        <oboInOwl:id>GAZ:00344430</oboInOwl:id>
        <rdfs:label>Bruckenbach</rdfs:label>
    </owl:NamedIndividual>
    


    <!-- http://purl.obolibrary.org/obo/GAZ_00344433 -->

    <owl:NamedIndividual rdf:about="http://purl.obolibrary.org/obo/GAZ_00344433">
        <obo:IAO_0000115>A river.</obo:IAO_0000115>
        <oboInOwl:hasOBONamespace>GAZ</oboInOwl:hasOBONamespace>
        <oboInOwl:id>GAZ:00344433</oboInOwl:id>
        <rdfs:label>Fassmattrunz</rdfs:label>
    </owl:NamedIndividual>
    


    <!-- http://purl.obolibrary.org/obo/GAZ_00344435 -->

    <owl:NamedIndividual rdf:about="http://purl.obolibrary.org/obo/GAZ_00344435">
        <obo:IAO_0000115>A river.</obo:IAO_0000115>
        <oboInOwl:hasOBONamespace>GAZ</oboInOwl:hasOBONamespace>
        <oboInOwl:id>GAZ:00344435</oboInOwl:id>
        <rdfs:label>Waldrunz</rdfs:label>
    </owl:NamedIndividual>
    


    <!-- http://purl.obolibrary.org/obo/GAZ_00344440 -->

    <owl:NamedIndividual rdf:about="http://purl.obolibrary.org/obo/GAZ_00344440">
        <obo:IAO_0000115>A river.</obo:IAO_0000115>
        <oboInOwl:hasOBONamespace>GAZ</oboInOwl:hasOBONamespace>
        <oboInOwl:id>GAZ:00344440</oboInOwl:id>
        <rdfs:label>Kuhlaegerunz</rdfs:label>
    </owl:NamedIndividual>
    


    <!-- http://purl.obolibrary.org/obo/GAZ_00344441 -->

    <owl:NamedIndividual rdf:about="http://purl.obolibrary.org/obo/GAZ_00344441">
        <obo:IAO_0000115>A river.</obo:IAO_0000115>
        <oboInOwl:hasOBONamespace>GAZ</oboInOwl:hasOBONamespace>
        <oboInOwl:id>GAZ:00344441</oboInOwl:id>
        <rdfs:label>Ruisseau le Kerlen</rdfs:label>
    </owl:NamedIndividual>
    


    <!-- http://purl.obolibrary.org/obo/GAZ_00344442 -->

    <owl:NamedIndividual rdf:about="http://purl.obolibrary.org/obo/GAZ_00344442">
        <obo:IAO_0000115>A river.</obo:IAO_0000115>
        <oboInOwl:hasOBONamespace>GAZ</oboInOwl:hasOBONamespace>
        <oboInOwl:id>GAZ:00344442</oboInOwl:id>
        <rdfs:label>Steinkloetz</rdfs:label>
    </owl:NamedIndividual>
    


    <!-- http://purl.obolibrary.org/obo/GAZ_00344443 -->

    <owl:NamedIndividual rdf:about="http://purl.obolibrary.org/obo/GAZ_00344443">
        <obo:IAO_0000115>A river.</obo:IAO_0000115>
        <oboInOwl:hasOBONamespace>GAZ</oboInOwl:hasOBONamespace>
        <oboInOwl:id>GAZ:00344443</oboInOwl:id>
        <rdfs:label>Ruisseau Allenbourn</rdfs:label>
    </owl:NamedIndividual>
    


    <!-- http://purl.obolibrary.org/obo/GAZ_00344444 -->

    <owl:NamedIndividual rdf:about="http://purl.obolibrary.org/obo/GAZ_00344444">
        <obo:IAO_0000115>A river.</obo:IAO_0000115>
        <oboInOwl:hasOBONamespace>GAZ</oboInOwl:hasOBONamespace>
        <oboInOwl:id>GAZ:00344444</oboInOwl:id>
        <rdfs:label>Grumbach</rdfs:label>
    </owl:NamedIndividual>
    


    <!-- http://purl.obolibrary.org/obo/GAZ_00344445 -->

    <owl:NamedIndividual rdf:about="http://purl.obolibrary.org/obo/GAZ_00344445">
        <obo:IAO_0000115>A river.</obo:IAO_0000115>
        <oboInOwl:hasOBONamespace>GAZ</oboInOwl:hasOBONamespace>
        <oboInOwl:id>GAZ:00344445</oboInOwl:id>
        <rdfs:label>Finsterbach</rdfs:label>
    </owl:NamedIndividual>
    


    <!-- http://purl.obolibrary.org/obo/GAZ_00344446 -->

    <owl:NamedIndividual rdf:about="http://purl.obolibrary.org/obo/GAZ_00344446">
        <obo:IAO_0000115>A dam. Impounds Lac de Kruth-Wildenstein.</obo:IAO_0000115>
        <oboInOwl:hasOBONamespace>GAZ</oboInOwl:hasOBONamespace>
        <oboInOwl:id>GAZ:00344446</oboInOwl:id>
        <rdfs:label>Barrage de Kruth-Wildenstein</rdfs:label>
    </owl:NamedIndividual>
    


    <!-- http://purl.obolibrary.org/obo/GAZ_00344490 -->

    <owl:NamedIndividual rdf:about="http://purl.obolibrary.org/obo/GAZ_00344490">
        <obo:IAO_0000115>A river.</obo:IAO_0000115>
        <oboInOwl:hasOBONamespace>GAZ</oboInOwl:hasOBONamespace>
        <oboInOwl:id>GAZ:00344490</oboInOwl:id>
        <rdfs:label>Durschbach</rdfs:label>
    </owl:NamedIndividual>
    


    <!-- http://purl.obolibrary.org/obo/GAZ_00344491 -->

    <owl:NamedIndividual rdf:about="http://purl.obolibrary.org/obo/GAZ_00344491">
        <obo:IAO_0000115>A river.</obo:IAO_0000115>
        <oboInOwl:hasOBONamespace>GAZ</oboInOwl:hasOBONamespace>
        <oboInOwl:id>GAZ:00344491</oboInOwl:id>
        <rdfs:label>Daetenbach</rdfs:label>
    </owl:NamedIndividual>
    


    <!-- http://purl.obolibrary.org/obo/GAZ_00344494 -->

    <owl:NamedIndividual rdf:about="http://purl.obolibrary.org/obo/GAZ_00344494">
        <obo:IAO_0000115>A river.</obo:IAO_0000115>
        <oboInOwl:hasOBONamespace>GAZ</oboInOwl:hasOBONamespace>
        <oboInOwl:id>GAZ:00344494</oboInOwl:id>
        <rdfs:label>Moderbach [Zinsel]</rdfs:label>
    </owl:NamedIndividual>
    


    <!-- http://purl.obolibrary.org/obo/GAZ_00344495 -->

    <owl:NamedIndividual rdf:about="http://purl.obolibrary.org/obo/GAZ_00344495">
        <obo:IAO_0000115>A river.</obo:IAO_0000115>
        <oboInOwl:hasOBONamespace>GAZ</oboInOwl:hasOBONamespace>
        <oboInOwl:id>GAZ:00344495</oboInOwl:id>
        <rdfs:label>Aar</rdfs:label>
    </owl:NamedIndividual>
    


    <!-- http://purl.obolibrary.org/obo/GAZ_00344529 -->

    <owl:NamedIndividual rdf:about="http://purl.obolibrary.org/obo/GAZ_00344529">
        <obo:IAO_0000115>A river.</obo:IAO_0000115>
        <oboInOwl:hasOBONamespace>GAZ</oboInOwl:hasOBONamespace>
        <oboInOwl:id>GAZ:00344529</oboInOwl:id>
        <rdfs:label>Meurthe</rdfs:label>
    </owl:NamedIndividual>
    


    <!-- http://purl.obolibrary.org/obo/GAZ_00360576 -->

    <owl:NamedIndividual rdf:about="http://purl.obolibrary.org/obo/GAZ_00360576">
        <obo:RO_0001025 rdf:resource="http://purl.obolibrary.org/obo/GAZ_00013815"/>
        <obo:IAO_0000115>A populated place.</obo:IAO_0000115>
        <oboInOwl:hasOBONamespace>GAZ</oboInOwl:hasOBONamespace>
        <oboInOwl:id>GAZ:00360576</oboInOwl:id>
        <rdfs:label>Balzers</rdfs:label>
    </owl:NamedIndividual>
    


    <!-- http://purl.obolibrary.org/obo/GAZ_00360577 -->

    <owl:NamedIndividual rdf:about="http://purl.obolibrary.org/obo/GAZ_00360577">
        <obo:RO_0001025 rdf:resource="http://purl.obolibrary.org/obo/GAZ_00013815"/>
        <obo:IAO_0000115>A populated place.</obo:IAO_0000115>
        <oboInOwl:hasOBONamespace>GAZ</oboInOwl:hasOBONamespace>
        <oboInOwl:id>GAZ:00360577</oboInOwl:id>
        <rdfs:label>Mals</rdfs:label>
    </owl:NamedIndividual>
    


    <!-- http://purl.obolibrary.org/obo/GAZ_00360578 -->

    <owl:NamedIndividual rdf:about="http://purl.obolibrary.org/obo/GAZ_00360578">
        <obo:RO_0001025 rdf:resource="http://purl.obolibrary.org/obo/GAZ_00013807"/>
        <obo:IAO_0000115>A populated place.</obo:IAO_0000115>
        <oboInOwl:hasOBONamespace>GAZ</oboInOwl:hasOBONamespace>
        <oboInOwl:id>GAZ:00360578</oboInOwl:id>
        <rdfs:label>Triesen</rdfs:label>
    </owl:NamedIndividual>
    


    <!-- http://purl.obolibrary.org/obo/GAZ_00360579 -->

    <owl:NamedIndividual rdf:about="http://purl.obolibrary.org/obo/GAZ_00360579">
        <obo:RO_0001025 rdf:resource="http://purl.obolibrary.org/obo/GAZ_00013812"/>
        <obo:IAO_0000115>A populated place.</obo:IAO_0000115>
        <oboInOwl:hasOBONamespace>GAZ</oboInOwl:hasOBONamespace>
        <oboInOwl:id>GAZ:00360579</oboInOwl:id>
        <rdfs:label>Triesenberg</rdfs:label>
    </owl:NamedIndividual>
    


    <!-- http://purl.obolibrary.org/obo/GAZ_00360580 -->

    <owl:NamedIndividual rdf:about="http://purl.obolibrary.org/obo/GAZ_00360580">
        <obo:RO_0001025 rdf:resource="http://purl.obolibrary.org/obo/GAZ_00013812"/>
        <obo:IAO_0000115>A populated place.</obo:IAO_0000115>
        <oboInOwl:hasOBONamespace>GAZ</oboInOwl:hasOBONamespace>
        <oboInOwl:id>GAZ:00360580</oboInOwl:id>
        <rdfs:label>Gaflei</rdfs:label>
    </owl:NamedIndividual>
    


    <!-- http://purl.obolibrary.org/obo/GAZ_00360581 -->

    <owl:NamedIndividual rdf:about="http://purl.obolibrary.org/obo/GAZ_00360581">
        <obo:RO_0001025 rdf:resource="http://purl.obolibrary.org/obo/GAZ_00013812"/>
        <obo:IAO_0000115>A populated place.</obo:IAO_0000115>
        <oboInOwl:hasOBONamespace>GAZ</oboInOwl:hasOBONamespace>
        <oboInOwl:id>GAZ:00360581</oboInOwl:id>
        <rdfs:label>Malbun</rdfs:label>
    </owl:NamedIndividual>
    


    <!-- http://purl.obolibrary.org/obo/GAZ_00360582 -->

    <owl:NamedIndividual rdf:about="http://purl.obolibrary.org/obo/GAZ_00360582">
        <obo:RO_0001025 rdf:resource="http://purl.obolibrary.org/obo/GAZ_00013812"/>
        <obo:IAO_0000115>A populated place.</obo:IAO_0000115>
        <oboInOwl:hasOBONamespace>GAZ</oboInOwl:hasOBONamespace>
        <oboInOwl:id>GAZ:00360582</oboInOwl:id>
        <rdfs:label>Masescha</rdfs:label>
    </owl:NamedIndividual>
    


    <!-- http://purl.obolibrary.org/obo/GAZ_00360583 -->

    <owl:NamedIndividual rdf:about="http://purl.obolibrary.org/obo/GAZ_00360583">
        <obo:RO_0001025 rdf:resource="http://purl.obolibrary.org/obo/GAZ_00013812"/>
        <obo:IAO_0000115>A populated place.</obo:IAO_0000115>
        <oboInOwl:hasOBONamespace>GAZ</oboInOwl:hasOBONamespace>
        <oboInOwl:id>GAZ:00360583</oboInOwl:id>
        <rdfs:label>Rotenboden</rdfs:label>
    </owl:NamedIndividual>
    


    <!-- http://purl.obolibrary.org/obo/GAZ_00360584 -->

    <owl:NamedIndividual rdf:about="http://purl.obolibrary.org/obo/GAZ_00360584">
        <obo:RO_0001025 rdf:resource="http://purl.obolibrary.org/obo/GAZ_00013812"/>
        <obo:IAO_0000115>A populated place.</obo:IAO_0000115>
        <oboInOwl:hasOBONamespace>GAZ</oboInOwl:hasOBONamespace>
        <oboInOwl:id>GAZ:00360584</oboInOwl:id>
        <rdfs:label>Samina</rdfs:label>
    </owl:NamedIndividual>
    


    <!-- http://purl.obolibrary.org/obo/GAZ_00360585 -->

    <owl:NamedIndividual rdf:about="http://purl.obolibrary.org/obo/GAZ_00360585">
        <obo:RO_0001025 rdf:resource="http://purl.obolibrary.org/obo/GAZ_00013812"/>
        <obo:IAO_0000115>A populated place.</obo:IAO_0000115>
        <oboInOwl:hasOBONamespace>GAZ</oboInOwl:hasOBONamespace>
        <oboInOwl:id>GAZ:00360585</oboInOwl:id>
        <rdfs:label>Silum</rdfs:label>
    </owl:NamedIndividual>
    


    <!-- http://purl.obolibrary.org/obo/GAZ_00360586 -->

    <owl:NamedIndividual rdf:about="http://purl.obolibrary.org/obo/GAZ_00360586">
        <obo:RO_0001025 rdf:resource="http://purl.obolibrary.org/obo/GAZ_00013812"/>
        <obo:IAO_0000115>A populated place.</obo:IAO_0000115>
        <oboInOwl:hasOBONamespace>GAZ</oboInOwl:hasOBONamespace>
        <oboInOwl:id>GAZ:00360586</oboInOwl:id>
        <rdfs:label>Steg</rdfs:label>
    </owl:NamedIndividual>
    


    <!-- http://purl.obolibrary.org/obo/GAZ_00360587 -->

    <owl:NamedIndividual rdf:about="http://purl.obolibrary.org/obo/GAZ_00360587">
        <obo:RO_0001025 rdf:resource="http://purl.obolibrary.org/obo/GAZ_00013812"/>
        <obo:IAO_0000115>A populated place.</obo:IAO_0000115>
        <oboInOwl:hasOBONamespace>GAZ</oboInOwl:hasOBONamespace>
        <oboInOwl:id>GAZ:00360587</oboInOwl:id>
        <rdfs:label>Sucka</rdfs:label>
    </owl:NamedIndividual>
    


    <!-- http://purl.obolibrary.org/obo/GAZ_00360588 -->

    <owl:NamedIndividual rdf:about="http://purl.obolibrary.org/obo/GAZ_00360588">
        <obo:RO_0001025 rdf:resource="http://purl.obolibrary.org/obo/GAZ_00013812"/>
        <obo:IAO_0000115>A populated place.</obo:IAO_0000115>
        <oboInOwl:hasOBONamespace>GAZ</oboInOwl:hasOBONamespace>
        <oboInOwl:id>GAZ:00360588</oboInOwl:id>
        <rdfs:label>Wangerberg</rdfs:label>
    </owl:NamedIndividual>
    


    <!-- http://purl.obolibrary.org/obo/GAZ_00360589 -->

    <owl:NamedIndividual rdf:about="http://purl.obolibrary.org/obo/GAZ_00360589">
        <obo:RO_0001025 rdf:resource="http://purl.obolibrary.org/obo/GAZ_00013809"/>
        <obo:IAO_0000115>A populated place.</obo:IAO_0000115>
        <oboInOwl:hasOBONamespace>GAZ</oboInOwl:hasOBONamespace>
        <oboInOwl:id>GAZ:00360589</oboInOwl:id>
        <rdfs:label>Vaduz</rdfs:label>
    </owl:NamedIndividual>
    


    <!-- http://purl.obolibrary.org/obo/GAZ_00360590 -->

    <owl:NamedIndividual rdf:about="http://purl.obolibrary.org/obo/GAZ_00360590">
        <obo:RO_0001025 rdf:resource="http://purl.obolibrary.org/obo/GAZ_00013809"/>
        <obo:IAO_0000115>A populated place.</obo:IAO_0000115>
        <oboInOwl:hasOBONamespace>GAZ</oboInOwl:hasOBONamespace>
        <oboInOwl:id>GAZ:00360590</oboInOwl:id>
        <rdfs:label>Ebenholz</rdfs:label>
    </owl:NamedIndividual>
    


    <!-- http://purl.obolibrary.org/obo/GAZ_00360591 -->

    <owl:NamedIndividual rdf:about="http://purl.obolibrary.org/obo/GAZ_00360591">
        <obo:RO_0001025 rdf:resource="http://purl.obolibrary.org/obo/GAZ_00013808"/>
        <obo:IAO_0000115>A populated place.</obo:IAO_0000115>
        <oboInOwl:hasOBONamespace>GAZ</oboInOwl:hasOBONamespace>
        <oboInOwl:id>GAZ:00360591</oboInOwl:id>
        <rdfs:label>Planken</rdfs:label>
    </owl:NamedIndividual>
    


    <!-- http://purl.obolibrary.org/obo/GAZ_00360592 -->

    <owl:NamedIndividual rdf:about="http://purl.obolibrary.org/obo/GAZ_00360592">
        <obo:RO_0001025 rdf:resource="http://purl.obolibrary.org/obo/GAZ_00013808"/>
        <obo:IAO_0000115>A populated place.</obo:IAO_0000115>
        <oboInOwl:hasOBONamespace>GAZ</oboInOwl:hasOBONamespace>
        <oboInOwl:id>GAZ:00360592</oboInOwl:id>
        <rdfs:label>Hinterschellenberg</rdfs:label>
    </owl:NamedIndividual>
    


    <!-- http://purl.obolibrary.org/obo/GAZ_00360593 -->

    <owl:NamedIndividual rdf:about="http://purl.obolibrary.org/obo/GAZ_00360593">
        <obo:RO_0001025 rdf:resource="http://purl.obolibrary.org/obo/GAZ_00013814"/>
        <obo:IAO_0000115>A populated place.</obo:IAO_0000115>
        <oboInOwl:hasOBONamespace>GAZ</oboInOwl:hasOBONamespace>
        <oboInOwl:id>GAZ:00360593</oboInOwl:id>
        <rdfs:label>Mauren</rdfs:label>
    </owl:NamedIndividual>
    


    <!-- http://purl.obolibrary.org/obo/GAZ_00360594 -->

    <owl:NamedIndividual rdf:about="http://purl.obolibrary.org/obo/GAZ_00360594">
        <obo:RO_0001025 rdf:resource="http://purl.obolibrary.org/obo/GAZ_00013811"/>
        <obo:IAO_0000115>A populated place.</obo:IAO_0000115>
        <oboInOwl:hasOBONamespace>GAZ</oboInOwl:hasOBONamespace>
        <oboInOwl:id>GAZ:00360594</oboInOwl:id>
        <rdfs:label>Eschen</rdfs:label>
    </owl:NamedIndividual>
    


    <!-- http://purl.obolibrary.org/obo/GAZ_00360595 -->

    <owl:NamedIndividual rdf:about="http://purl.obolibrary.org/obo/GAZ_00360595">
        <obo:RO_0001025 rdf:resource="http://purl.obolibrary.org/obo/GAZ_00013811"/>
        <obo:IAO_0000115>A populated place.</obo:IAO_0000115>
        <oboInOwl:hasOBONamespace>GAZ</oboInOwl:hasOBONamespace>
        <oboInOwl:id>GAZ:00360595</oboInOwl:id>
        <rdfs:label>Nendeln</rdfs:label>
    </owl:NamedIndividual>
    


    <!-- http://purl.obolibrary.org/obo/GAZ_00360596 -->

    <owl:NamedIndividual rdf:about="http://purl.obolibrary.org/obo/GAZ_00360596">
        <obo:RO_0001025 rdf:resource="http://purl.obolibrary.org/obo/GAZ_00013805"/>
        <obo:IAO_0000115>A populated place.</obo:IAO_0000115>
        <oboInOwl:hasOBONamespace>GAZ</oboInOwl:hasOBONamespace>
        <oboInOwl:id>GAZ:00360596</oboInOwl:id>
        <rdfs:label>Gamprin</rdfs:label>
    </owl:NamedIndividual>
    


    <!-- http://purl.obolibrary.org/obo/GAZ_00360597 -->

    <owl:NamedIndividual rdf:about="http://purl.obolibrary.org/obo/GAZ_00360597">
        <obo:RO_0001025 rdf:resource="http://purl.obolibrary.org/obo/GAZ_00013805"/>
        <obo:IAO_0000115>A populated place.</obo:IAO_0000115>
        <oboInOwl:hasOBONamespace>GAZ</oboInOwl:hasOBONamespace>
        <oboInOwl:id>GAZ:00360597</oboInOwl:id>
        <rdfs:label>Bendern</rdfs:label>
    </owl:NamedIndividual>
    


    <!-- http://purl.obolibrary.org/obo/GAZ_00360598 -->

    <owl:NamedIndividual rdf:about="http://purl.obolibrary.org/obo/GAZ_00360598">
        <obo:RO_0001025 rdf:resource="http://purl.obolibrary.org/obo/GAZ_00013813"/>
        <obo:IAO_0000115>A populated place.</obo:IAO_0000115>
        <oboInOwl:hasOBONamespace>GAZ</oboInOwl:hasOBONamespace>
        <oboInOwl:id>GAZ:00360598</oboInOwl:id>
        <rdfs:label>Schellenberg</rdfs:label>
    </owl:NamedIndividual>
    


    <!-- http://purl.obolibrary.org/obo/GAZ_00360599 -->

    <owl:NamedIndividual rdf:about="http://purl.obolibrary.org/obo/GAZ_00360599">
        <obo:RO_0001025 rdf:resource="http://purl.obolibrary.org/obo/GAZ_00013810"/>
        <obo:IAO_0000115>A populated place.</obo:IAO_0000115>
        <oboInOwl:hasOBONamespace>GAZ</oboInOwl:hasOBONamespace>
        <oboInOwl:id>GAZ:00360599</oboInOwl:id>
        <rdfs:label>Ruggell</rdfs:label>
    </owl:NamedIndividual>
    


    <!-- http://purl.obolibrary.org/obo/GAZ_00378648 -->

    <owl:NamedIndividual rdf:about="http://purl.obolibrary.org/obo/GAZ_00378648">
        <obo:IAO_0000115>A lake.</obo:IAO_0000115>
        <oboInOwl:hasOBONamespace>GAZ</oboInOwl:hasOBONamespace>
        <oboInOwl:id>GAZ:00378648</oboInOwl:id>
        <rdfs:label>Gajseva Lake</rdfs:label>
    </owl:NamedIndividual>
    


    <!-- http://purl.obolibrary.org/obo/GAZ_00378650 -->

    <owl:NamedIndividual rdf:about="http://purl.obolibrary.org/obo/GAZ_00378650">
        <obo:RO_0001025 rdf:resource="http://purl.obolibrary.org/obo/GAZ_00051916"/>
        <obo:IAO_0000115>A mountain range, part of the Southern Limestone Alps in north Slovenia and at the border with Austria.</obo:IAO_0000115>
        <oboInOwl:hasOBONamespace>GAZ</oboInOwl:hasOBONamespace>
        <oboInOwl:id>GAZ:00378650</oboInOwl:id>
        <rdfs:label>Kamnik-Savinja Alps</rdfs:label>
    </owl:NamedIndividual>
    


    <!-- http://purl.obolibrary.org/obo/GAZ_00378651 -->

    <owl:NamedIndividual rdf:about="http://purl.obolibrary.org/obo/GAZ_00378651">
        <obo:RO_0001025 rdf:resource="http://purl.obolibrary.org/obo/GAZ_00378650"/>
        <obo:IAO_0000115>A mountain range.</obo:IAO_0000115>
        <oboInOwl:hasOBONamespace>GAZ</oboInOwl:hasOBONamespace>
        <oboInOwl:id>GAZ:00378651</oboInOwl:id>
        <rdfs:label>Savinja Alps</rdfs:label>
    </owl:NamedIndividual>
    


    <!-- http://purl.obolibrary.org/obo/GAZ_00378652 -->

    <owl:NamedIndividual rdf:about="http://purl.obolibrary.org/obo/GAZ_00378652">
        <obo:RO_0001025 rdf:resource="http://purl.obolibrary.org/obo/GAZ_00056804"/>
        <obo:IAO_0000115>A mountain peak.</obo:IAO_0000115>
        <oboInOwl:hasOBONamespace>GAZ</oboInOwl:hasOBONamespace>
        <oboInOwl:id>GAZ:00378652</oboInOwl:id>
        <rdfs:label>Skuta</rdfs:label>
    </owl:NamedIndividual>
    


    <!-- http://purl.obolibrary.org/obo/GAZ_00378653 -->

    <owl:NamedIndividual rdf:about="http://purl.obolibrary.org/obo/GAZ_00378653">
        <obo:RO_0001025 rdf:resource="http://purl.obolibrary.org/obo/GAZ_00378652"/>
        <obo:IAO_0000115>A glacier.</obo:IAO_0000115>
        <oboInOwl:hasOBONamespace>GAZ</oboInOwl:hasOBONamespace>
        <oboInOwl:id>GAZ:00378653</oboInOwl:id>
        <rdfs:label>Skuta Glacier</rdfs:label>
    </owl:NamedIndividual>
    


    <!-- http://purl.obolibrary.org/obo/GAZ_00378671 -->

    <owl:NamedIndividual rdf:about="http://purl.obolibrary.org/obo/GAZ_00378671">
        <obo:IAO_0000115>A river. It flows through western Slovenia and northeast Italy. Discharges to the Adriatic Sea.</obo:IAO_0000115>
        <oboInOwl:hasOBONamespace>GAZ</oboInOwl:hasOBONamespace>
        <oboInOwl:id>GAZ:00378671</oboInOwl:id>
        <rdfs:label>Soca</rdfs:label>
    </owl:NamedIndividual>
    


    <!-- http://purl.obolibrary.org/obo/GAZ_00390517 -->

    <owl:NamedIndividual rdf:about="http://purl.obolibrary.org/obo/GAZ_00390517">
        <obo:IAO_0000115>A river. Discharges to the Mediterranean Sea.</obo:IAO_0000115>
        <oboInOwl:hasOBONamespace>GAZ</oboInOwl:hasOBONamespace>
        <oboInOwl:id>GAZ:00390517</oboInOwl:id>
        <rdfs:label>Huveaune</rdfs:label>
    </owl:NamedIndividual>
    


    <!-- http://purl.obolibrary.org/obo/GAZ_00391175 -->

    <owl:NamedIndividual rdf:about="http://purl.obolibrary.org/obo/GAZ_00391175">
        <obo:RO_0001025 rdf:resource="http://purl.obolibrary.org/obo/GAZ_00006787"/>
        <obo:IAO_0000115>A protected area.</obo:IAO_0000115>
        <oboInOwl:hasOBONamespace>GAZ</oboInOwl:hasOBONamespace>
        <oboInOwl:id>GAZ:00391175</oboInOwl:id>
        <rdfs:label>Parc naturel regional du Luberon</rdfs:label>
    </owl:NamedIndividual>
    


    <!-- http://purl.obolibrary.org/obo/GAZ_00391398 -->

    <owl:NamedIndividual rdf:about="http://purl.obolibrary.org/obo/GAZ_00391398">
        <obo:IAO_0000115>A reservoir. Constructed 1979.</obo:IAO_0000115>
        <oboInOwl:hasOBONamespace>GAZ</oboInOwl:hasOBONamespace>
        <oboInOwl:id>GAZ:00391398</oboInOwl:id>
        <rdfs:label>Stausei Uewersauer</rdfs:label>
    </owl:NamedIndividual>
    


    <!-- http://purl.obolibrary.org/obo/GAZ_00391442 -->

    <owl:NamedIndividual rdf:about="http://purl.obolibrary.org/obo/GAZ_00391442">
        <obo:RO_0001025 rdf:resource="http://purl.obolibrary.org/obo/GAZ_00060584"/>
        <obo:IAO_0000115>A glacier. Located on the northern slopes of the Mont Blanc massif.</obo:IAO_0000115>
        <oboInOwl:hasOBONamespace>GAZ</oboInOwl:hasOBONamespace>
        <oboInOwl:id>GAZ:00391442</oboInOwl:id>
        <rdfs:label>Mer de Glace</rdfs:label>
    </owl:NamedIndividual>
    


    <!-- http://purl.obolibrary.org/obo/GAZ_00393369 -->

    <owl:NamedIndividual rdf:about="http://purl.obolibrary.org/obo/GAZ_00393369">
        <rdf:type rdf:resource="http://purl.obolibrary.org/obo/ENVO_00000100"/>
        <obo:RO_0001025 rdf:resource="http://purl.obolibrary.org/obo/GAZ_00060581"/>
        <obo:IAO_0000115>A gorge.</obo:IAO_0000115>
        <oboInOwl:hasOBONamespace>GAZ</oboInOwl:hasOBONamespace>
        <oboInOwl:id>GAZ:00393369</oboInOwl:id>
        <rdfs:label>Gorges du Pont-du-Diable</rdfs:label>
    </owl:NamedIndividual>
    


    <!-- http://purl.obolibrary.org/obo/GAZ_00393420 -->

    <owl:NamedIndividual rdf:about="http://purl.obolibrary.org/obo/GAZ_00393420">
        <obo:RO_0001025 rdf:resource="http://purl.obolibrary.org/obo/GAZ_00060591"/>
        <obo:IAO_0000115>A karst cave system.</obo:IAO_0000115>
        <oboInOwl:hasOBONamespace>GAZ</oboInOwl:hasOBONamespace>
        <oboInOwl:id>GAZ:00393420</oboInOwl:id>
        <rdfs:label>Vercors Cave System</rdfs:label>
    </owl:NamedIndividual>
    


    <!-- http://purl.obolibrary.org/obo/GAZ_00393421 -->

    <owl:NamedIndividual rdf:about="http://purl.obolibrary.org/obo/GAZ_00393421">
        <obo:RO_0001025 rdf:resource="http://purl.obolibrary.org/obo/GAZ_00393420"/>
        <obo:IAO_0000115>A cave. The entrance is within the commune of Engins high on the Vercors Plateau.</obo:IAO_0000115>
        <oboInOwl:hasOBONamespace>GAZ</oboInOwl:hasOBONamespace>
        <oboInOwl:id>GAZ:00393421</oboInOwl:id>
        <rdfs:label>Gouffre Berger</rdfs:label>
    </owl:NamedIndividual>
    


    <!-- http://purl.obolibrary.org/obo/GAZ_00393423 -->

    <owl:NamedIndividual rdf:about="http://purl.obolibrary.org/obo/GAZ_00393423">
        <rdf:type rdf:resource="http://purl.obolibrary.org/obo/ENVO_00000100"/>
        <obo:RO_0001025 rdf:resource="http://purl.obolibrary.org/obo/GAZ_00060591"/>
        <obo:IAO_0000115>A gorge.</obo:IAO_0000115>
        <oboInOwl:hasOBONamespace>GAZ</oboInOwl:hasOBONamespace>
        <oboInOwl:id>GAZ:00393423</oboInOwl:id>
        <rdfs:label>Gorges de la Bourne</rdfs:label>
    </owl:NamedIndividual>
    


    <!-- http://purl.obolibrary.org/obo/GAZ_00393492 -->

    <owl:NamedIndividual rdf:about="http://purl.obolibrary.org/obo/GAZ_00393492">
        <obo:RO_0001025 rdf:resource="http://purl.obolibrary.org/obo/GAZ_00060591"/>
        <obo:IAO_0000115>A cave system.</obo:IAO_0000115>
        <oboInOwl:hasOBONamespace>GAZ</oboInOwl:hasOBONamespace>
        <oboInOwl:id>GAZ:00393492</oboInOwl:id>
        <rdfs:label>Les Cuves de Sassenage</rdfs:label>
    </owl:NamedIndividual>
    


    <!-- http://purl.obolibrary.org/obo/GAZ_00393509 -->

    <owl:NamedIndividual rdf:about="http://purl.obolibrary.org/obo/GAZ_00393509">
        <obo:RO_0001025 rdf:resource="http://purl.obolibrary.org/obo/GAZ_00060577"/>
        <obo:IAO_0000115>A lake.</obo:IAO_0000115>
        <oboInOwl:hasOBONamespace>GAZ</oboInOwl:hasOBONamespace>
        <oboInOwl:id>GAZ:00393509</oboInOwl:id>
        <rdfs:label>Lac de l&apos;Aiguillete</rdfs:label>
    </owl:NamedIndividual>
    


    <!-- http://purl.obolibrary.org/obo/GAZ_00393510 -->

    <owl:NamedIndividual rdf:about="http://purl.obolibrary.org/obo/GAZ_00393510">
        <obo:RO_0001025 rdf:resource="http://purl.obolibrary.org/obo/GAZ_00060577"/>
        <obo:IAO_0000115>A protected area.</obo:IAO_0000115>
        <oboInOwl:hasOBONamespace>GAZ</oboInOwl:hasOBONamespace>
        <oboInOwl:id>GAZ:00393510</oboInOwl:id>
        <rdfs:label>Reserve naturelle nationale des Aiguilles Rouges</rdfs:label>
    </owl:NamedIndividual>
    


    <!-- http://purl.obolibrary.org/obo/GAZ_00393511 -->

    <owl:NamedIndividual rdf:about="http://purl.obolibrary.org/obo/GAZ_00393511">
        <obo:RO_0001025 rdf:resource="http://purl.obolibrary.org/obo/GAZ_00060577"/>
        <obo:IAO_0000115>A protected area.</obo:IAO_0000115>
        <oboInOwl:hasOBONamespace>GAZ</oboInOwl:hasOBONamespace>
        <oboInOwl:id>GAZ:00393511</oboInOwl:id>
        <rdfs:label>Reserve naturelle de Passy</rdfs:label>
    </owl:NamedIndividual>
    


    <!-- http://purl.obolibrary.org/obo/GAZ_00393512 -->

    <owl:NamedIndividual rdf:about="http://purl.obolibrary.org/obo/GAZ_00393512">
        <obo:RO_0001025 rdf:resource="http://purl.obolibrary.org/obo/GAZ_00060584"/>
        <obo:IAO_0000115>A glacier.</obo:IAO_0000115>
        <oboInOwl:hasOBONamespace>GAZ</oboInOwl:hasOBONamespace>
        <oboInOwl:id>GAZ:00393512</oboInOwl:id>
        <rdfs:label>Glacier d&apos;Argentiere</rdfs:label>
    </owl:NamedIndividual>
    


    <!-- http://purl.obolibrary.org/obo/GAZ_00393513 -->

    <owl:NamedIndividual rdf:about="http://purl.obolibrary.org/obo/GAZ_00393513">
        <obo:RO_0001025 rdf:resource="http://purl.obolibrary.org/obo/GAZ_00060584"/>
        <obo:IAO_0000115>A glacier.</obo:IAO_0000115>
        <oboInOwl:hasOBONamespace>GAZ</oboInOwl:hasOBONamespace>
        <oboInOwl:id>GAZ:00393513</oboInOwl:id>
        <rdfs:label>Glacier des Bossons</rdfs:label>
    </owl:NamedIndividual>
    


    <!-- http://purl.obolibrary.org/obo/GAZ_00393514 -->

    <owl:NamedIndividual rdf:about="http://purl.obolibrary.org/obo/GAZ_00393514">
        <obo:RO_0001025 rdf:resource="http://purl.obolibrary.org/obo/GAZ_00060584"/>
        <obo:IAO_0000115>A debris-covered glacier in northwestern Italy. It is situated on the southwest flank of the Mont Blanc massif, flowing from Col de Bionnassay (3892m above sea level) into Val Veny.</obo:IAO_0000115>
        <oboInOwl:hasOBONamespace>GAZ</oboInOwl:hasOBONamespace>
        <oboInOwl:id>GAZ:00393514</oboInOwl:id>
        <rdfs:label>Glacier du Miage</rdfs:label>
    </owl:NamedIndividual>
    


    <!-- http://purl.obolibrary.org/obo/GAZ_00393515 -->

    <owl:NamedIndividual rdf:about="http://purl.obolibrary.org/obo/GAZ_00393515">
        <obo:RO_0001025 rdf:resource="http://purl.obolibrary.org/obo/GAZ_00393514"/>
        <obo:IAO_0000115>An ice-contact lake near the southern end of the Miage Glacier.</obo:IAO_0000115>
        <oboInOwl:hasOBONamespace>GAZ</oboInOwl:hasOBONamespace>
        <oboInOwl:id>GAZ:00393515</oboInOwl:id>
        <rdfs:label>Miage Lake</rdfs:label>
    </owl:NamedIndividual>
    


    <!-- http://purl.obolibrary.org/obo/GAZ_00393516 -->

    <owl:NamedIndividual rdf:about="http://purl.obolibrary.org/obo/GAZ_00393516">
        <obo:RO_0001025 rdf:resource="http://purl.obolibrary.org/obo/GAZ_00060584"/>
        <obo:IAO_0000115>A glacier situated in the Mont Blanc Massif in the canton of Valais in Switzerland.</obo:IAO_0000115>
        <oboInOwl:hasOBONamespace>GAZ</oboInOwl:hasOBONamespace>
        <oboInOwl:id>GAZ:00393516</oboInOwl:id>
        <rdfs:label>Glacier du Trient</rdfs:label>
    </owl:NamedIndividual>
    


    <!-- http://purl.obolibrary.org/obo/GAZ_00393518 -->

    <owl:NamedIndividual rdf:about="http://purl.obolibrary.org/obo/GAZ_00393518">
        <obo:IAO_0000115>A river.</obo:IAO_0000115>
        <oboInOwl:hasOBONamespace>GAZ</oboInOwl:hasOBONamespace>
        <oboInOwl:id>GAZ:00393518</oboInOwl:id>
        <rdfs:label>Arveyron</rdfs:label>
    </owl:NamedIndividual>
    


    <!-- http://purl.obolibrary.org/obo/GAZ_00393560 -->

    <owl:NamedIndividual rdf:about="http://purl.obolibrary.org/obo/GAZ_00393560">
        <obo:RO_0001025 rdf:resource="http://purl.obolibrary.org/obo/GAZ_00060577"/>
        <obo:IAO_0000115>A protected area.</obo:IAO_0000115>
        <oboInOwl:hasOBONamespace>GAZ</oboInOwl:hasOBONamespace>
        <oboInOwl:id>GAZ:00393560</oboInOwl:id>
        <rdfs:label>Reserve naturelle des Contamines-Montjoie</rdfs:label>
    </owl:NamedIndividual>
    


    <!-- http://purl.obolibrary.org/obo/GAZ_00394501 -->

    <owl:NamedIndividual rdf:about="http://purl.obolibrary.org/obo/GAZ_00394501">
        <obo:RO_0001025 rdf:resource="http://purl.obolibrary.org/obo/GAZ_00393423"/>
        <obo:IAO_0000115>Karst caves.</obo:IAO_0000115>
        <oboInOwl:hasOBONamespace>GAZ</oboInOwl:hasOBONamespace>
        <oboInOwl:id>GAZ:00394501</oboInOwl:id>
        <rdfs:label>Grottes de Choranche</rdfs:label>
    </owl:NamedIndividual>
    


    <!-- http://purl.obolibrary.org/obo/GAZ_00396725 -->

    <owl:NamedIndividual rdf:about="http://purl.obolibrary.org/obo/GAZ_00396725">
        <obo:RO_0001025 rdf:resource="http://purl.obolibrary.org/obo/GAZ_00060608"/>
        <obo:IAO_0000115>A lake.</obo:IAO_0000115>
        <oboInOwl:hasOBONamespace>GAZ</oboInOwl:hasOBONamespace>
        <oboInOwl:id>GAZ:00396725</oboInOwl:id>
        <rdfs:label>Lac Long</rdfs:label>
    </owl:NamedIndividual>
    


    <!-- http://purl.obolibrary.org/obo/GAZ_00403300 -->

    <owl:NamedIndividual rdf:about="http://purl.obolibrary.org/obo/GAZ_00403300">
        <obo:IAO_0000115>A river.</obo:IAO_0000115>
        <oboInOwl:hasOBONamespace>GAZ</oboInOwl:hasOBONamespace>
        <oboInOwl:id>GAZ:00403300</oboInOwl:id>
        <rdfs:label>Waschgraben</rdfs:label>
    </owl:NamedIndividual>
    


    <!-- http://purl.obolibrary.org/obo/GAZ_00406382 -->

    <owl:NamedIndividual rdf:about="http://purl.obolibrary.org/obo/GAZ_00406382">
        <obo:RO_0001025 rdf:resource="http://purl.obolibrary.org/obo/GAZ_00060591"/>
        <obo:IAO_0000115>A karst field.</obo:IAO_0000115>
        <oboInOwl:hasOBONamespace>GAZ</oboInOwl:hasOBONamespace>
        <oboInOwl:id>GAZ:00406382</oboInOwl:id>
        <rdfs:label>Plateau de Vassieux</rdfs:label>
    </owl:NamedIndividual>
    


    <!-- http://purl.obolibrary.org/obo/GAZ_00408717 -->

    <owl:NamedIndividual rdf:about="http://purl.obolibrary.org/obo/GAZ_00408717">
        <obo:RO_0001025 rdf:resource="http://purl.obolibrary.org/obo/GAZ_00060256"/>
        <obo:IAO_0000115>A glacial valley.</obo:IAO_0000115>
        <oboInOwl:hasOBONamespace>GAZ</oboInOwl:hasOBONamespace>
        <oboInOwl:id>GAZ:00408717</oboInOwl:id>
        <rdfs:label>Valgaudemar</rdfs:label>
    </owl:NamedIndividual>
    


    <!-- http://purl.obolibrary.org/obo/GAZ_00408747 -->

    <owl:NamedIndividual rdf:about="http://purl.obolibrary.org/obo/GAZ_00408747">
        <obo:RO_0001025 rdf:resource="http://purl.obolibrary.org/obo/GAZ_00408717"/>
        <obo:IAO_0000115>A glacier.</obo:IAO_0000115>
        <oboInOwl:hasOBONamespace>GAZ</oboInOwl:hasOBONamespace>
        <oboInOwl:id>GAZ:00408747</oboInOwl:id>
        <rdfs:label>Glacier de l&apos;Aup</rdfs:label>
    </owl:NamedIndividual>
    


    <!-- http://purl.obolibrary.org/obo/GAZ_00408749 -->

    <owl:NamedIndividual rdf:about="http://purl.obolibrary.org/obo/GAZ_00408749">
        <obo:RO_0001025 rdf:resource="http://purl.obolibrary.org/obo/GAZ_00408717"/>
        <obo:IAO_0000115>A glacier.</obo:IAO_0000115>
        <oboInOwl:hasOBONamespace>GAZ</oboInOwl:hasOBONamespace>
        <oboInOwl:id>GAZ:00408749</oboInOwl:id>
        <rdfs:label>Glacier de Crupillouse</rdfs:label>
    </owl:NamedIndividual>
    


    <!-- http://purl.obolibrary.org/obo/GAZ_00408750 -->

    <owl:NamedIndividual rdf:about="http://purl.obolibrary.org/obo/GAZ_00408750">
        <obo:RO_0001025 rdf:resource="http://purl.obolibrary.org/obo/GAZ_00060256"/>
        <obo:IAO_0000115>A glacier.</obo:IAO_0000115>
        <oboInOwl:hasOBONamespace>GAZ</oboInOwl:hasOBONamespace>
        <oboInOwl:id>GAZ:00408750</oboInOwl:id>
        <rdfs:label>Glacier d&apos;Arsine</rdfs:label>
    </owl:NamedIndividual>
    


    <!-- http://purl.obolibrary.org/obo/GAZ_00408752 -->

    <owl:NamedIndividual rdf:about="http://purl.obolibrary.org/obo/GAZ_00408752">
        <obo:RO_0001025 rdf:resource="http://purl.obolibrary.org/obo/GAZ_00060256"/>
        <obo:IAO_0000115>A glacier.</obo:IAO_0000115>
        <oboInOwl:hasOBONamespace>GAZ</oboInOwl:hasOBONamespace>
        <oboInOwl:id>GAZ:00408752</oboInOwl:id>
        <rdfs:label>Glacier Blanc</rdfs:label>
    </owl:NamedIndividual>
    


    <!-- http://purl.obolibrary.org/obo/GAZ_00408755 -->

    <owl:NamedIndividual rdf:about="http://purl.obolibrary.org/obo/GAZ_00408755">
        <obo:RO_0001025 rdf:resource="http://purl.obolibrary.org/obo/GAZ_00008405"/>
        <obo:RO_0001025 rdf:resource="http://purl.obolibrary.org/obo/GAZ_00060209"/>
        <obo:IAO_0000115>A mountain massif.</obo:IAO_0000115>
        <oboInOwl:hasOBONamespace>GAZ</oboInOwl:hasOBONamespace>
        <oboInOwl:id>GAZ:00408755</oboInOwl:id>
        <rdfs:label>Massif du Queyras</rdfs:label>
    </owl:NamedIndividual>
    


    <!-- http://purl.obolibrary.org/obo/GAZ_00411073 -->

    <owl:NamedIndividual rdf:about="http://purl.obolibrary.org/obo/GAZ_00411073">
        <obo:RO_0001025 rdf:resource="http://purl.obolibrary.org/obo/GAZ_00060580"/>
        <obo:IAO_0000115>A plateau.</obo:IAO_0000115>
        <oboInOwl:hasOBONamespace>GAZ</oboInOwl:hasOBONamespace>
        <oboInOwl:id>GAZ:00411073</oboInOwl:id>
        <rdfs:label>Plateau des Glieres</rdfs:label>
    </owl:NamedIndividual>
    


    <!-- http://purl.obolibrary.org/obo/GAZ_00411138 -->

    <owl:NamedIndividual rdf:about="http://purl.obolibrary.org/obo/GAZ_00411138">
        <obo:IAO_0000115>A river.</obo:IAO_0000115>
        <oboInOwl:hasOBONamespace>GAZ</oboInOwl:hasOBONamespace>
        <oboInOwl:id>GAZ:00411138</oboInOwl:id>
        <rdfs:label>Torrent du Chapeau</rdfs:label>
    </owl:NamedIndividual>
    


    <!-- http://purl.obolibrary.org/obo/GAZ_00411146 -->

    <owl:NamedIndividual rdf:about="http://purl.obolibrary.org/obo/GAZ_00411146">
        <obo:IAO_0000115>A hydroelectric dam. Constructed 1967-1972.</obo:IAO_0000115>
        <oboInOwl:hasOBONamespace>GAZ</oboInOwl:hasOBONamespace>
        <oboInOwl:id>GAZ:00411146</oboInOwl:id>
        <rdfs:label>Barrage d&apos;Emosson</rdfs:label>
    </owl:NamedIndividual>
    


    <!-- http://purl.obolibrary.org/obo/GAZ_00411147 -->

    <owl:NamedIndividual rdf:about="http://purl.obolibrary.org/obo/GAZ_00411147">
        <obo:IAO_0000115>A river.</obo:IAO_0000115>
        <oboInOwl:hasOBONamespace>GAZ</oboInOwl:hasOBONamespace>
        <oboInOwl:id>GAZ:00411147</oboInOwl:id>
        <rdfs:label>Ruisseau de la Duche</rdfs:label>
    </owl:NamedIndividual>
    


    <!-- http://purl.obolibrary.org/obo/GAZ_00411148 -->

    <owl:NamedIndividual rdf:about="http://purl.obolibrary.org/obo/GAZ_00411148">
        <obo:IAO_0000115>A river.</obo:IAO_0000115>
        <oboInOwl:hasOBONamespace>GAZ</oboInOwl:hasOBONamespace>
        <oboInOwl:id>GAZ:00411148</oboInOwl:id>
        <rdfs:label>Torrent de Chinaillon</rdfs:label>
    </owl:NamedIndividual>
    


    <!-- http://purl.obolibrary.org/obo/GAZ_00411149 -->

    <owl:NamedIndividual rdf:about="http://purl.obolibrary.org/obo/GAZ_00411149">
        <obo:IAO_0000115>A river.</obo:IAO_0000115>
        <oboInOwl:hasOBONamespace>GAZ</oboInOwl:hasOBONamespace>
        <oboInOwl:id>GAZ:00411149</oboInOwl:id>
        <rdfs:label>Overan</rdfs:label>
    </owl:NamedIndividual>
    


    <!-- http://purl.obolibrary.org/obo/GAZ_00411150 -->

    <owl:NamedIndividual rdf:about="http://purl.obolibrary.org/obo/GAZ_00411150">
        <obo:IAO_0000115>A river.</obo:IAO_0000115>
        <oboInOwl:hasOBONamespace>GAZ</oboInOwl:hasOBONamespace>
        <oboInOwl:id>GAZ:00411150</oboInOwl:id>
        <rdfs:label>Ruisseau du Grand Nant</rdfs:label>
    </owl:NamedIndividual>
    


    <!-- http://purl.obolibrary.org/obo/GAZ_00411151 -->

    <owl:NamedIndividual rdf:about="http://purl.obolibrary.org/obo/GAZ_00411151">
        <obo:IAO_0000115>A river.</obo:IAO_0000115>
        <oboInOwl:hasOBONamespace>GAZ</oboInOwl:hasOBONamespace>
        <oboInOwl:id>GAZ:00411151</oboInOwl:id>
        <rdfs:label>Ruisseau des Combes</rdfs:label>
    </owl:NamedIndividual>
    


    <!-- http://purl.obolibrary.org/obo/GAZ_00411152 -->

    <owl:NamedIndividual rdf:about="http://purl.obolibrary.org/obo/GAZ_00411152">
        <obo:IAO_0000115>A river.</obo:IAO_0000115>
        <oboInOwl:hasOBONamespace>GAZ</oboInOwl:hasOBONamespace>
        <oboInOwl:id>GAZ:00411152</oboInOwl:id>
        <rdfs:label>Ruisseau Nant de la Ville</rdfs:label>
    </owl:NamedIndividual>
    


    <!-- http://purl.obolibrary.org/obo/GAZ_00411153 -->

    <owl:NamedIndividual rdf:about="http://purl.obolibrary.org/obo/GAZ_00411153">
        <obo:IAO_0000115>A river.</obo:IAO_0000115>
        <oboInOwl:hasOBONamespace>GAZ</oboInOwl:hasOBONamespace>
        <oboInOwl:id>GAZ:00411153</oboInOwl:id>
        <rdfs:label>Ruisseau Nant du Talave</rdfs:label>
    </owl:NamedIndividual>
    


    <!-- http://purl.obolibrary.org/obo/GAZ_00411154 -->

    <owl:NamedIndividual rdf:about="http://purl.obolibrary.org/obo/GAZ_00411154">
        <obo:IAO_0000115>A river.</obo:IAO_0000115>
        <oboInOwl:hasOBONamespace>GAZ</oboInOwl:hasOBONamespace>
        <oboInOwl:id>GAZ:00411154</oboInOwl:id>
        <rdfs:label>Torrent Jalandre</rdfs:label>
    </owl:NamedIndividual>
    


    <!-- http://purl.obolibrary.org/obo/GAZ_00411155 -->

    <owl:NamedIndividual rdf:about="http://purl.obolibrary.org/obo/GAZ_00411155">
        <obo:IAO_0000115>A river.</obo:IAO_0000115>
        <oboInOwl:hasOBONamespace>GAZ</oboInOwl:hasOBONamespace>
        <oboInOwl:id>GAZ:00411155</oboInOwl:id>
        <rdfs:label>Ruisseau de la Dresse</rdfs:label>
    </owl:NamedIndividual>
    


    <!-- http://purl.obolibrary.org/obo/GAZ_00411156 -->

    <owl:NamedIndividual rdf:about="http://purl.obolibrary.org/obo/GAZ_00411156">
        <obo:IAO_0000115>A river.</obo:IAO_0000115>
        <oboInOwl:hasOBONamespace>GAZ</oboInOwl:hasOBONamespace>
        <oboInOwl:id>GAZ:00411156</oboInOwl:id>
        <rdfs:label>Ruisseau de Beffay</rdfs:label>
    </owl:NamedIndividual>
    


    <!-- http://purl.obolibrary.org/obo/GAZ_00411157 -->

    <owl:NamedIndividual rdf:about="http://purl.obolibrary.org/obo/GAZ_00411157">
        <obo:IAO_0000115>A river.</obo:IAO_0000115>
        <oboInOwl:hasOBONamespace>GAZ</oboInOwl:hasOBONamespace>
        <oboInOwl:id>GAZ:00411157</oboInOwl:id>
        <rdfs:label>Ruisseau du Taleu</rdfs:label>
    </owl:NamedIndividual>
    


    <!-- http://purl.obolibrary.org/obo/GAZ_00411158 -->

    <owl:NamedIndividual rdf:about="http://purl.obolibrary.org/obo/GAZ_00411158">
        <obo:IAO_0000115>A river.</obo:IAO_0000115>
        <oboInOwl:hasOBONamespace>GAZ</oboInOwl:hasOBONamespace>
        <oboInOwl:id>GAZ:00411158</oboInOwl:id>
        <rdfs:label>Le Delairaz</rdfs:label>
    </owl:NamedIndividual>
    


    <!-- http://purl.obolibrary.org/obo/GAZ_00411228 -->

    <owl:NamedIndividual rdf:about="http://purl.obolibrary.org/obo/GAZ_00411228">
        <obo:IAO_0000115>A river. A headwater of the Sallanche.</obo:IAO_0000115>
        <oboInOwl:hasOBONamespace>GAZ</oboInOwl:hasOBONamespace>
        <oboInOwl:id>GAZ:00411228</oboInOwl:id>
        <rdfs:label>Ruisseau du Brayon</rdfs:label>
    </owl:NamedIndividual>
    


    <!-- http://purl.obolibrary.org/obo/GAZ_00419214 -->

    <owl:NamedIndividual rdf:about="http://purl.obolibrary.org/obo/GAZ_00419214">
        <obo:RO_0001025 rdf:resource="http://purl.obolibrary.org/obo/GAZ_00060579"/>
        <obo:IAO_0000115>A protected area.</obo:IAO_0000115>
        <oboInOwl:hasOBONamespace>GAZ</oboInOwl:hasOBONamespace>
        <oboInOwl:id>GAZ:00419214</oboInOwl:id>
        <rdfs:label>Reserve naturelle des Hauts de Chartreuse</rdfs:label>
    </owl:NamedIndividual>
    


    <!-- http://purl.obolibrary.org/obo/GAZ_00419215 -->

    <owl:NamedIndividual rdf:about="http://purl.obolibrary.org/obo/GAZ_00419215">
        <obo:RO_0001025 rdf:resource="http://purl.obolibrary.org/obo/GAZ_00060591"/>
        <obo:IAO_0000115>A protected area. Established 1970.</obo:IAO_0000115>
        <oboInOwl:hasOBONamespace>GAZ</oboInOwl:hasOBONamespace>
        <oboInOwl:id>GAZ:00419215</oboInOwl:id>
        <rdfs:label>Reserve naturelle des Hauts plateaux du Vercors</rdfs:label>
    </owl:NamedIndividual>
    


    <!-- http://purl.obolibrary.org/obo/GAZ_00419218 -->

    <owl:NamedIndividual rdf:about="http://purl.obolibrary.org/obo/GAZ_00419218">
        <obo:RO_0001025 rdf:resource="http://purl.obolibrary.org/obo/GAZ_00060579"/>
        <obo:IAO_0000115>A forest.</obo:IAO_0000115>
        <oboInOwl:hasOBONamespace>GAZ</oboInOwl:hasOBONamespace>
        <oboInOwl:id>GAZ:00419218</oboInOwl:id>
        <rdfs:label>Foret de la Grande Chartreuse</rdfs:label>
    </owl:NamedIndividual>
    


    <!-- http://purl.obolibrary.org/obo/GAZ_00419219 -->

    <owl:NamedIndividual rdf:about="http://purl.obolibrary.org/obo/GAZ_00419219">
        <obo:RO_0001025 rdf:resource="http://purl.obolibrary.org/obo/GAZ_00060391"/>
        <obo:IAO_0000115>A glacier.</obo:IAO_0000115>
        <oboInOwl:hasOBONamespace>GAZ</oboInOwl:hasOBONamespace>
        <oboInOwl:id>GAZ:00419219</oboInOwl:id>
        <rdfs:label>Glacier de Freydane</rdfs:label>
    </owl:NamedIndividual>
    


    <!-- http://purl.obolibrary.org/obo/GAZ_00419220 -->

    <owl:NamedIndividual rdf:about="http://purl.obolibrary.org/obo/GAZ_00419220">
        <obo:RO_0001025 rdf:resource="http://purl.obolibrary.org/obo/GAZ_00060256"/>
        <obo:IAO_0000115>A glacial lake.</obo:IAO_0000115>
        <oboInOwl:hasOBONamespace>GAZ</oboInOwl:hasOBONamespace>
        <oboInOwl:id>GAZ:00419220</oboInOwl:id>
        <rdfs:label>Lac des Beches</rdfs:label>
    </owl:NamedIndividual>
    


    <!-- http://purl.obolibrary.org/obo/GAZ_00419255 -->

    <owl:NamedIndividual rdf:about="http://purl.obolibrary.org/obo/GAZ_00419255">
        <obo:RO_0001025 rdf:resource="http://purl.obolibrary.org/obo/GAZ_00060391"/>
        <obo:IAO_0000115>Three lakes.</obo:IAO_0000115>
        <oboInOwl:hasOBONamespace>GAZ</oboInOwl:hasOBONamespace>
        <oboInOwl:id>GAZ:00419255</oboInOwl:id>
        <rdfs:label>Lacs Robert</rdfs:label>
    </owl:NamedIndividual>
    


    <!-- http://purl.obolibrary.org/obo/GAZ_00419256 -->

    <owl:NamedIndividual rdf:about="http://purl.obolibrary.org/obo/GAZ_00419256">
        <obo:RO_0001025 rdf:resource="http://purl.obolibrary.org/obo/GAZ_00419255"/>
        <obo:IAO_0000115>A lake.</obo:IAO_0000115>
        <oboInOwl:hasOBONamespace>GAZ</oboInOwl:hasOBONamespace>
        <oboInOwl:id>GAZ:00419256</oboInOwl:id>
        <rdfs:label>Lac Robert petite sud</rdfs:label>
    </owl:NamedIndividual>
    


    <!-- http://purl.obolibrary.org/obo/GAZ_00419257 -->

    <owl:NamedIndividual rdf:about="http://purl.obolibrary.org/obo/GAZ_00419257">
        <obo:RO_0001025 rdf:resource="http://purl.obolibrary.org/obo/GAZ_00419255"/>
        <obo:IAO_0000115>A lake.</obo:IAO_0000115>
        <oboInOwl:hasOBONamespace>GAZ</oboInOwl:hasOBONamespace>
        <oboInOwl:id>GAZ:00419257</oboInOwl:id>
        <rdfs:label>Lac Robert petite nord</rdfs:label>
    </owl:NamedIndividual>
    


    <!-- http://purl.obolibrary.org/obo/GAZ_00419258 -->

    <owl:NamedIndividual rdf:about="http://purl.obolibrary.org/obo/GAZ_00419258">
        <obo:RO_0001025 rdf:resource="http://purl.obolibrary.org/obo/GAZ_00060391"/>
        <obo:RO_0001025 rdf:resource="http://purl.obolibrary.org/obo/GAZ_00419255"/>
        <oboInOwl:hasOBONamespace>GAZ</oboInOwl:hasOBONamespace>
        <oboInOwl:id>GAZ:00419258</oboInOwl:id>
        <rdfs:label>Grand Lac Robert</rdfs:label>
    </owl:NamedIndividual>
    


    <!-- http://purl.obolibrary.org/obo/GAZ_00419259 -->

    <owl:NamedIndividual rdf:about="http://purl.obolibrary.org/obo/GAZ_00419259">
        <obo:RO_0001025 rdf:resource="http://purl.obolibrary.org/obo/GAZ_00060256"/>
        <obo:IAO_0000115>A glacial lake.</obo:IAO_0000115>
        <oboInOwl:hasOBONamespace>GAZ</oboInOwl:hasOBONamespace>
        <oboInOwl:id>GAZ:00419259</oboInOwl:id>
        <rdfs:label>Lac des Rouies</rdfs:label>
    </owl:NamedIndividual>
    


    <!-- http://purl.obolibrary.org/obo/GAZ_00419394 -->

    <owl:NamedIndividual rdf:about="http://purl.obolibrary.org/obo/GAZ_00419394">
        <obo:IAO_0000115>A river.</obo:IAO_0000115>
        <oboInOwl:hasOBONamespace>GAZ</oboInOwl:hasOBONamespace>
        <oboInOwl:id>GAZ:00419394</oboInOwl:id>
        <rdfs:label>Loux</rdfs:label>
    </owl:NamedIndividual>
    


    <!-- http://purl.obolibrary.org/obo/GAZ_00419395 -->

    <owl:NamedIndividual rdf:about="http://purl.obolibrary.org/obo/GAZ_00419395">
        <obo:IAO_0000115>A river.</obo:IAO_0000115>
        <oboInOwl:hasOBONamespace>GAZ</oboInOwl:hasOBONamespace>
        <oboInOwl:id>GAZ:00419395</oboInOwl:id>
        <rdfs:label>Ruisseau de l&apos;Achard</rdfs:label>
    </owl:NamedIndividual>
    


    <!-- http://purl.obolibrary.org/obo/GAZ_00419396 -->

    <owl:NamedIndividual rdf:about="http://purl.obolibrary.org/obo/GAZ_00419396">
        <obo:IAO_0000115>A river.</obo:IAO_0000115>
        <oboInOwl:hasOBONamespace>GAZ</oboInOwl:hasOBONamespace>
        <oboInOwl:id>GAZ:00419396</oboInOwl:id>
        <rdfs:label>Ruisseau de Sarcenas</rdfs:label>
    </owl:NamedIndividual>
    


    <!-- http://purl.obolibrary.org/obo/GAZ_00419397 -->

    <owl:NamedIndividual rdf:about="http://purl.obolibrary.org/obo/GAZ_00419397">
        <obo:IAO_0000115>A river.</obo:IAO_0000115>
        <oboInOwl:hasOBONamespace>GAZ</oboInOwl:hasOBONamespace>
        <oboInOwl:id>GAZ:00419397</oboInOwl:id>
        <rdfs:label>Ruisseau des Groules</rdfs:label>
    </owl:NamedIndividual>
    


    <!-- http://purl.obolibrary.org/obo/GAZ_00419398 -->

    <owl:NamedIndividual rdf:about="http://purl.obolibrary.org/obo/GAZ_00419398">
        <obo:IAO_0000115>A river.</obo:IAO_0000115>
        <oboInOwl:hasOBONamespace>GAZ</oboInOwl:hasOBONamespace>
        <oboInOwl:id>GAZ:00419398</oboInOwl:id>
        <rdfs:label>Coleon</rdfs:label>
    </owl:NamedIndividual>
    


    <!-- http://purl.obolibrary.org/obo/GAZ_00419399 -->

    <owl:NamedIndividual rdf:about="http://purl.obolibrary.org/obo/GAZ_00419399">
        <obo:IAO_0000115>A river.</obo:IAO_0000115>
        <oboInOwl:hasOBONamespace>GAZ</oboInOwl:hasOBONamespace>
        <oboInOwl:id>GAZ:00419399</oboInOwl:id>
        <rdfs:label>Tenaison</rdfs:label>
    </owl:NamedIndividual>
    


    <!-- http://purl.obolibrary.org/obo/GAZ_00423841 -->

    <owl:NamedIndividual rdf:about="http://purl.obolibrary.org/obo/GAZ_00423841">
        <obo:IAO_0000115>A tunnel.</obo:IAO_0000115>
        <oboInOwl:hasOBONamespace>GAZ</oboInOwl:hasOBONamespace>
        <oboInOwl:id>GAZ:00423841</oboInOwl:id>
        <rdfs:label>Tunnel de Mauvages</rdfs:label>
    </owl:NamedIndividual>
    


    <!-- http://purl.obolibrary.org/obo/GAZ_00424894 -->

    <owl:NamedIndividual rdf:about="http://purl.obolibrary.org/obo/GAZ_00424894">
        <obo:IAO_0000115>A river.</obo:IAO_0000115>
        <oboInOwl:hasOBONamespace>GAZ</oboInOwl:hasOBONamespace>
        <oboInOwl:id>GAZ:00424894</oboInOwl:id>
        <rdfs:label>Oude Schelde</rdfs:label>
    </owl:NamedIndividual>
    


    <!-- http://purl.obolibrary.org/obo/GAZ_00425282 -->

    <owl:NamedIndividual rdf:about="http://purl.obolibrary.org/obo/GAZ_00425282">
        <obo:RO_0001025 rdf:resource="http://purl.obolibrary.org/obo/GAZ_00179752"/>
        <obo:IAO_0000115>A protected area. A polder.</obo:IAO_0000115>
        <oboInOwl:hasOBONamespace>GAZ</oboInOwl:hasOBONamespace>
        <oboInOwl:id>GAZ:00425282</oboInOwl:id>
        <rdfs:label>Lippenbroek</rdfs:label>
    </owl:NamedIndividual>
    


    <!-- http://purl.obolibrary.org/obo/GAZ_00426950 -->

    <owl:NamedIndividual rdf:about="http://purl.obolibrary.org/obo/GAZ_00426950">
        <obo:IAO_0000115>A river port.</obo:IAO_0000115>
        <oboInOwl:hasOBONamespace>GAZ</oboInOwl:hasOBONamespace>
        <oboInOwl:id>GAZ:00426950</oboInOwl:id>
        <rdfs:label>Port autonome de Liege</rdfs:label>
    </owl:NamedIndividual>
    


    <!-- http://purl.obolibrary.org/obo/GAZ_00427964 -->

    <owl:NamedIndividual rdf:about="http://purl.obolibrary.org/obo/GAZ_00427964">
        <obo:IAO_0000115>A canal.</obo:IAO_0000115>
        <oboInOwl:hasOBONamespace>GAZ</oboInOwl:hasOBONamespace>
        <oboInOwl:id>GAZ:00427964</oboInOwl:id>
        <rdfs:label>Verbindingskanaal</rdfs:label>
    </owl:NamedIndividual>
    


    <!-- http://purl.obolibrary.org/obo/GAZ_00427965 -->

    <owl:NamedIndividual rdf:about="http://purl.obolibrary.org/obo/GAZ_00427965">
        <obo:IAO_0000115>A canal.</obo:IAO_0000115>
        <oboInOwl:hasOBONamespace>GAZ</oboInOwl:hasOBONamespace>
        <oboInOwl:id>GAZ:00427965</oboInOwl:id>
        <rdfs:label>Coupure</rdfs:label>
    </owl:NamedIndividual>
    


    <!-- http://purl.obolibrary.org/obo/GAZ_00430386 -->

    <owl:NamedIndividual rdf:about="http://purl.obolibrary.org/obo/GAZ_00430386">
        <obo:RO_0001025 rdf:resource="http://purl.obolibrary.org/obo/GAZ_00060579"/>
        <obo:IAO_0000115>A mountain; a protected area.</obo:IAO_0000115>
        <oboInOwl:hasOBONamespace>GAZ</oboInOwl:hasOBONamespace>
        <oboInOwl:id>GAZ:00430386</oboInOwl:id>
        <rdfs:label>Mont Outheran</rdfs:label>
    </owl:NamedIndividual>
    


    <!-- http://purl.obolibrary.org/obo/GAZ_00430387 -->

    <owl:NamedIndividual rdf:about="http://purl.obolibrary.org/obo/GAZ_00430387">
        <obo:RO_0001025 rdf:resource="http://purl.obolibrary.org/obo/GAZ_00060579"/>
        <obo:IAO_0000115>A mountain; a protected area.</obo:IAO_0000115>
        <oboInOwl:hasOBONamespace>GAZ</oboInOwl:hasOBONamespace>
        <oboInOwl:id>GAZ:00430387</oboInOwl:id>
        <rdfs:label>Mont Joigny</rdfs:label>
    </owl:NamedIndividual>
    


    <!-- http://purl.obolibrary.org/obo/GAZ_00430389 -->

    <owl:NamedIndividual rdf:about="http://purl.obolibrary.org/obo/GAZ_00430389">
        <obo:RO_0001025 rdf:resource="http://purl.obolibrary.org/obo/GAZ_00060578"/>
        <obo:IAO_0000115>A glacial cirque.</obo:IAO_0000115>
        <oboInOwl:hasOBONamespace>GAZ</oboInOwl:hasOBONamespace>
        <oboInOwl:id>GAZ:00430389</oboInOwl:id>
        <rdfs:label>Le Bout du Monde</rdfs:label>
    </owl:NamedIndividual>
    


    <!-- http://purl.obolibrary.org/obo/GAZ_00430390 -->

    <owl:NamedIndividual rdf:about="http://purl.obolibrary.org/obo/GAZ_00430390">
        <obo:RO_0001025 rdf:resource="http://purl.obolibrary.org/obo/GAZ_00060578"/>
        <obo:IAO_0000115>A mountain massif.</obo:IAO_0000115>
        <oboInOwl:hasOBONamespace>GAZ</oboInOwl:hasOBONamespace>
        <oboInOwl:id>GAZ:00430390</oboInOwl:id>
        <rdfs:label>Massif du Haut-Giffre</rdfs:label>
    </owl:NamedIndividual>
    


    <!-- http://purl.obolibrary.org/obo/GAZ_00430391 -->

    <owl:NamedIndividual rdf:about="http://purl.obolibrary.org/obo/GAZ_00430391">
        <obo:RO_0001025 rdf:resource="http://purl.obolibrary.org/obo/GAZ_00060578"/>
        <obo:IAO_0000115>A mountain massif.</obo:IAO_0000115>
        <oboInOwl:hasOBONamespace>GAZ</oboInOwl:hasOBONamespace>
        <oboInOwl:id>GAZ:00430391</oboInOwl:id>
        <rdfs:label>Massif de Sixt</rdfs:label>
    </owl:NamedIndividual>
    


    <!-- http://purl.obolibrary.org/obo/GAZ_00430392 -->

    <owl:NamedIndividual rdf:about="http://purl.obolibrary.org/obo/GAZ_00430392">
        <obo:RO_0001025 rdf:resource="http://purl.obolibrary.org/obo/GAZ_00060578"/>
        <obo:IAO_0000115>A mountain massif.</obo:IAO_0000115>
        <oboInOwl:hasOBONamespace>GAZ</oboInOwl:hasOBONamespace>
        <oboInOwl:id>GAZ:00430392</oboInOwl:id>
        <rdfs:label>Massif du Faucigny</rdfs:label>
    </owl:NamedIndividual>
    


    <!-- http://purl.obolibrary.org/obo/GAZ_00430394 -->

    <owl:NamedIndividual rdf:about="http://purl.obolibrary.org/obo/GAZ_00430394">
        <obo:RO_0001025 rdf:resource="http://purl.obolibrary.org/obo/GAZ_00419214"/>
        <obo:IAO_0000115>A cirque.</obo:IAO_0000115>
        <oboInOwl:hasOBONamespace>GAZ</oboInOwl:hasOBONamespace>
        <oboInOwl:id>GAZ:00430394</oboInOwl:id>
        <rdfs:label>Cirque de Saint-Meme</rdfs:label>
    </owl:NamedIndividual>
    


    <!-- http://purl.obolibrary.org/obo/GAZ_00431988 -->

    <owl:NamedIndividual rdf:about="http://purl.obolibrary.org/obo/GAZ_00431988">
        <rdf:type rdf:resource="http://purl.obolibrary.org/obo/ENVO_00000080"/>
        <obo:RO_0001025 rdf:resource="http://purl.obolibrary.org/obo/GAZ_00060598"/>
        <obo:IAO_0000115>A mountain chain.</obo:IAO_0000115>
        <oboInOwl:hasOBONamespace>GAZ</oboInOwl:hasOBONamespace>
        <oboInOwl:id>GAZ:00431988</oboInOwl:id>
        <rdfs:label>Les Cuguyons</rdfs:label>
    </owl:NamedIndividual>
    


    <!-- http://purl.obolibrary.org/obo/GAZ_00432296 -->

    <owl:NamedIndividual rdf:about="http://purl.obolibrary.org/obo/GAZ_00432296">
        <obo:IAO_0000115>A man-made lake. Constructed 1983.</obo:IAO_0000115>
        <oboInOwl:hasOBONamespace>GAZ</oboInOwl:hasOBONamespace>
        <oboInOwl:id>GAZ:00432296</oboInOwl:id>
        <rdfs:label>Lac de la Lande</rdfs:label>
    </owl:NamedIndividual>
    


    <!-- http://purl.obolibrary.org/obo/GAZ_00595587 -->

    <owl:NamedIndividual rdf:about="http://purl.obolibrary.org/obo/GAZ_00595587">
        <obo:IAO_0000115>A pump-storage hydroelectric power station.</obo:IAO_0000115>
        <oboInOwl:hasOBONamespace>GAZ</oboInOwl:hasOBONamespace>
        <oboInOwl:id>GAZ:00595587</oboInOwl:id>
        <rdfs:label>Rudolf-Fettweis-Werk</rdfs:label>
    </owl:NamedIndividual>
    


    <!-- http://purl.obolibrary.org/obo/GAZ_00595588 -->

    <owl:NamedIndividual rdf:about="http://purl.obolibrary.org/obo/GAZ_00595588">
        <obo:RO_0001025 rdf:resource="http://purl.obolibrary.org/obo/GAZ_00595587"/>
        <obo:IAO_0000115>A dam and associated resevoir.</obo:IAO_0000115>
        <oboInOwl:hasOBONamespace>GAZ</oboInOwl:hasOBONamespace>
        <oboInOwl:id>GAZ:00595588</oboInOwl:id>
        <rdfs:label>Schwarzenbachtalsperre</rdfs:label>
    </owl:NamedIndividual>
    


    <!-- http://purl.obolibrary.org/obo/GAZ_00595591 -->

    <owl:NamedIndividual rdf:about="http://purl.obolibrary.org/obo/GAZ_00595591">
        <obo:RO_0001025 rdf:resource="http://purl.obolibrary.org/obo/GAZ_00008262"/>
        <obo:IAO_0000115>A lock. The two passages of the lock serve to allow ships and barges to bypass the hydropower station on the French side of the river.</obo:IAO_0000115>
        <oboInOwl:hasOBONamespace>GAZ</oboInOwl:hasOBONamespace>
        <oboInOwl:id>GAZ:00595591</oboInOwl:id>
        <rdfs:label>Schleuse Iffezheim</rdfs:label>
    </owl:NamedIndividual>
    


    <!-- http://purl.obolibrary.org/obo/GAZ_00595700 -->

    <owl:NamedIndividual rdf:about="http://purl.obolibrary.org/obo/GAZ_00595700">
        <obo:IAO_0000115>A harbor.</obo:IAO_0000115>
        <oboInOwl:hasOBONamespace>GAZ</oboInOwl:hasOBONamespace>
        <oboInOwl:id>GAZ:00595700</oboInOwl:id>
        <rdfs:label>Hafen 1 Handelshafen</rdfs:label>
    </owl:NamedIndividual>
    


    <!-- http://purl.obolibrary.org/obo/GAZ_00595701 -->

    <owl:NamedIndividual rdf:about="http://purl.obolibrary.org/obo/GAZ_00595701">
        <obo:IAO_0000115>A harbor.</obo:IAO_0000115>
        <oboInOwl:hasOBONamespace>GAZ</oboInOwl:hasOBONamespace>
        <oboInOwl:id>GAZ:00595701</oboInOwl:id>
        <rdfs:label>Hafen 2 Rheinauhafen</rdfs:label>
    </owl:NamedIndividual>
    


    <!-- http://purl.obolibrary.org/obo/GAZ_00595702 -->

    <owl:NamedIndividual rdf:about="http://purl.obolibrary.org/obo/GAZ_00595702">
        <obo:IAO_0000115>A harbor.</obo:IAO_0000115>
        <oboInOwl:hasOBONamespace>GAZ</oboInOwl:hasOBONamespace>
        <oboInOwl:id>GAZ:00595702</oboInOwl:id>
        <rdfs:label>Hafen 3 Altrheinhafen</rdfs:label>
    </owl:NamedIndividual>
    


    <!-- http://purl.obolibrary.org/obo/GAZ_00595703 -->

    <owl:NamedIndividual rdf:about="http://purl.obolibrary.org/obo/GAZ_00595703">
        <obo:IAO_0000115>A harbor.</obo:IAO_0000115>
        <oboInOwl:hasOBONamespace>GAZ</oboInOwl:hasOBONamespace>
        <oboInOwl:id>GAZ:00595703</oboInOwl:id>
        <rdfs:label>Hafen 4 Industriehafe</rdfs:label>
    </owl:NamedIndividual>
    


    <!-- http://purl.obolibrary.org/obo/GAZ_00595723 -->

    <owl:NamedIndividual rdf:about="http://purl.obolibrary.org/obo/GAZ_00595723">
        <rdf:type rdf:resource="http://purl.obolibrary.org/obo/ENVO_00000423"/>
        <obo:IAO_0000115>A fluvial island.</obo:IAO_0000115>
        <oboInOwl:hasOBONamespace>GAZ</oboInOwl:hasOBONamespace>
        <oboInOwl:id>GAZ:00595723</oboInOwl:id>
        <rdfs:label>Muhleninsel</rdfs:label>
    </owl:NamedIndividual>
    


    <!-- http://purl.obolibrary.org/obo/GAZ_00595724 -->

    <owl:NamedIndividual rdf:about="http://purl.obolibrary.org/obo/GAZ_00595724">
        <rdf:type rdf:resource="http://purl.obolibrary.org/obo/ENVO_00000423"/>
        <obo:IAO_0000115>A fluvial island.</obo:IAO_0000115>
        <oboInOwl:hasOBONamespace>GAZ</oboInOwl:hasOBONamespace>
        <oboInOwl:id>GAZ:00595724</oboInOwl:id>
        <rdfs:label>Museumsinsel</rdfs:label>
    </owl:NamedIndividual>
    


    <!-- http://purl.obolibrary.org/obo/GAZ_00595725 -->

    <owl:NamedIndividual rdf:about="http://purl.obolibrary.org/obo/GAZ_00595725">
        <rdf:type rdf:resource="http://purl.obolibrary.org/obo/ENVO_00000423"/>
        <obo:IAO_0000115>A fluvial island.</obo:IAO_0000115>
        <oboInOwl:hasOBONamespace>GAZ</oboInOwl:hasOBONamespace>
        <oboInOwl:id>GAZ:00595725</oboInOwl:id>
        <rdfs:label>Praterinsel</rdfs:label>
    </owl:NamedIndividual>
    


    <!-- http://purl.obolibrary.org/obo/GAZ_00596145 -->

    <owl:NamedIndividual rdf:about="http://purl.obolibrary.org/obo/GAZ_00596145">
        <obo:IAO_0000115>A dam and associated reservoir.</obo:IAO_0000115>
        <oboInOwl:hasOBONamespace>GAZ</oboInOwl:hasOBONamespace>
        <oboInOwl:id>GAZ:00596145</oboInOwl:id>
        <rdfs:label>Nagoldtalsperre</rdfs:label>
    </owl:NamedIndividual>
    


    <!-- http://purl.obolibrary.org/obo/GAZ_00597436 -->

    <owl:NamedIndividual rdf:about="http://purl.obolibrary.org/obo/GAZ_00597436">
        <obo:IAO_0000115>A river.</obo:IAO_0000115>
        <oboInOwl:hasOBONamespace>GAZ</oboInOwl:hasOBONamespace>
        <oboInOwl:id>GAZ:00597436</oboInOwl:id>
        <rdfs:label>Waschbach</rdfs:label>
    </owl:NamedIndividual>
    


    <!-- http://purl.obolibrary.org/obo/GAZ_00597437 -->

    <owl:NamedIndividual rdf:about="http://purl.obolibrary.org/obo/GAZ_00597437">
        <obo:IAO_0000115>A river.</obo:IAO_0000115>
        <oboInOwl:hasOBONamespace>GAZ</oboInOwl:hasOBONamespace>
        <oboInOwl:id>GAZ:00597437</oboInOwl:id>
        <rdfs:label>Dobach</rdfs:label>
    </owl:NamedIndividual>
    


    <!-- http://purl.obolibrary.org/obo/GAZ_00597438 -->

    <owl:NamedIndividual rdf:about="http://purl.obolibrary.org/obo/GAZ_00597438">
        <obo:IAO_0000115>A river.</obo:IAO_0000115>
        <oboInOwl:hasOBONamespace>GAZ</oboInOwl:hasOBONamespace>
        <oboInOwl:id>GAZ:00597438</oboInOwl:id>
        <rdfs:label>Lauter [Mogglingen]</rdfs:label>
    </owl:NamedIndividual>
    


    <!-- http://purl.obolibrary.org/obo/GAZ_00598050 -->

    <owl:NamedIndividual rdf:about="http://purl.obolibrary.org/obo/GAZ_00598050">
        <obo:IAO_0000115>A pump storage dam.</obo:IAO_0000115>
        <oboInOwl:hasOBONamespace>GAZ</oboInOwl:hasOBONamespace>
        <oboInOwl:id>GAZ:00598050</oboInOwl:id>
        <rdfs:label>Schwarzatalsperre</rdfs:label>
    </owl:NamedIndividual>
    


    <!-- http://purl.obolibrary.org/obo/GAZ_00598057 -->

    <owl:NamedIndividual rdf:about="http://purl.obolibrary.org/obo/GAZ_00598057">
        <obo:IAO_0000115>A protected area.</obo:IAO_0000115>
        <oboInOwl:hasOBONamespace>GAZ</oboInOwl:hasOBONamespace>
        <oboInOwl:id>GAZ:00598057</oboInOwl:id>
        <rdfs:label>Naturschutzgebiet Bodenseeufer (Bodman-Ludwigshafen)</rdfs:label>
    </owl:NamedIndividual>
    


    <!-- http://purl.obolibrary.org/obo/GAZ_00598058 -->

    <owl:NamedIndividual rdf:about="http://purl.obolibrary.org/obo/GAZ_00598058">
        <obo:IAO_0000115>A protected area.</obo:IAO_0000115>
        <oboInOwl:hasOBONamespace>GAZ</oboInOwl:hasOBONamespace>
        <oboInOwl:id>GAZ:00598058</oboInOwl:id>
        <rdfs:label>Naturschutzgebiet Bodenseeufer (Konstanz)</rdfs:label>
    </owl:NamedIndividual>
    


    <!-- http://purl.obolibrary.org/obo/GAZ_00598059 -->

    <owl:NamedIndividual rdf:about="http://purl.obolibrary.org/obo/GAZ_00598059">
        <obo:IAO_0000115>A protected area.</obo:IAO_0000115>
        <oboInOwl:hasOBONamespace>GAZ</oboInOwl:hasOBONamespace>
        <oboInOwl:id>GAZ:00598059</oboInOwl:id>
        <rdfs:label>Naturschutzgebiet Bodenseeufer auf Gemarkung Markelfingen</rdfs:label>
    </owl:NamedIndividual>
    


    <!-- http://purl.obolibrary.org/obo/GAZ_00598060 -->

    <owl:NamedIndividual rdf:about="http://purl.obolibrary.org/obo/GAZ_00598060">
        <obo:IAO_0000115>A protected area.</obo:IAO_0000115>
        <oboInOwl:hasOBONamespace>GAZ</oboInOwl:hasOBONamespace>
        <oboInOwl:id>GAZ:00598060</oboInOwl:id>
        <rdfs:label>Naturschutzgebiet Bodenseeufer - Untere Gull</rdfs:label>
    </owl:NamedIndividual>
    


    <!-- http://purl.obolibrary.org/obo/GAZ_00598075 -->

    <owl:NamedIndividual rdf:about="http://purl.obolibrary.org/obo/GAZ_00598075">
        <obo:RO_0001025 rdf:resource="http://purl.obolibrary.org/obo/GAZ_00043216"/>
        <obo:IAO_0000115>A village (Dorf).</obo:IAO_0000115>
        <oboInOwl:hasOBONamespace>GAZ</oboInOwl:hasOBONamespace>
        <oboInOwl:id>GAZ:00598075</oboInOwl:id>
        <rdfs:label>Oberzell</rdfs:label>
    </owl:NamedIndividual>
    


    <!-- http://purl.obolibrary.org/obo/GAZ_00598076 -->

    <owl:NamedIndividual rdf:about="http://purl.obolibrary.org/obo/GAZ_00598076">
        <obo:RO_0001025 rdf:resource="http://purl.obolibrary.org/obo/GAZ_00043216"/>
        <obo:IAO_0000115>A village (Dorf).</obo:IAO_0000115>
        <oboInOwl:hasOBONamespace>GAZ</oboInOwl:hasOBONamespace>
        <oboInOwl:id>GAZ:00598076</oboInOwl:id>
        <rdfs:label>Mittelzell</rdfs:label>
    </owl:NamedIndividual>
    


    <!-- http://purl.obolibrary.org/obo/GAZ_00598077 -->

    <owl:NamedIndividual rdf:about="http://purl.obolibrary.org/obo/GAZ_00598077">
        <obo:RO_0001025 rdf:resource="http://purl.obolibrary.org/obo/GAZ_00043216"/>
        <obo:IAO_0000115>A village (Dorf).</obo:IAO_0000115>
        <oboInOwl:hasOBONamespace>GAZ</oboInOwl:hasOBONamespace>
        <oboInOwl:id>GAZ:00598077</oboInOwl:id>
        <rdfs:label>Niederzell</rdfs:label>
    </owl:NamedIndividual>
    


    <!-- http://purl.obolibrary.org/obo/GAZ_00598080 -->

    <owl:NamedIndividual rdf:about="http://purl.obolibrary.org/obo/GAZ_00598080">
        <obo:RO_0001025 rdf:resource="http://purl.obolibrary.org/obo/GAZ_00008111"/>
        <obo:IAO_0000115>A lacustrine island.</obo:IAO_0000115>
        <oboInOwl:hasOBONamespace>GAZ</oboInOwl:hasOBONamespace>
        <oboInOwl:id>GAZ:00598080</oboInOwl:id>
        <rdfs:label>Liebesinsel</rdfs:label>
    </owl:NamedIndividual>
    


    <!-- http://purl.obolibrary.org/obo/GAZ_00598087 -->

    <owl:NamedIndividual rdf:about="http://purl.obolibrary.org/obo/GAZ_00598087">
        <obo:RO_0001025 rdf:resource="http://purl.obolibrary.org/obo/GAZ_00058618"/>
        <obo:IAO_0000115>A bay.</obo:IAO_0000115>
        <oboInOwl:hasOBONamespace>GAZ</oboInOwl:hasOBONamespace>
        <oboInOwl:id>GAZ:00598087</oboInOwl:id>
        <rdfs:label>Konstanzer Trichter</rdfs:label>
    </owl:NamedIndividual>
    


    <!-- http://purl.obolibrary.org/obo/GAZ_00598089 -->

    <owl:NamedIndividual rdf:about="http://purl.obolibrary.org/obo/GAZ_00598089">
        <obo:RO_0001025 rdf:resource="http://purl.obolibrary.org/obo/GAZ_00058616"/>
        <obo:IAO_0000115>A lacustrine island.</obo:IAO_0000115>
        <oboInOwl:hasOBONamespace>GAZ</oboInOwl:hasOBONamespace>
        <oboInOwl:id>GAZ:00598089</oboInOwl:id>
        <rdfs:label>Triboldingerbohl</rdfs:label>
    </owl:NamedIndividual>
    


    <!-- http://purl.obolibrary.org/obo/GAZ_00598090 -->

    <owl:NamedIndividual rdf:about="http://purl.obolibrary.org/obo/GAZ_00598090">
        <obo:RO_0001025 rdf:resource="http://purl.obolibrary.org/obo/GAZ_00058616"/>
        <obo:IAO_0000115>A lacustrine island.</obo:IAO_0000115>
        <oboInOwl:hasOBONamespace>GAZ</oboInOwl:hasOBONamespace>
        <oboInOwl:id>GAZ:00598090</oboInOwl:id>
        <rdfs:label>Mittler Bohl</rdfs:label>
    </owl:NamedIndividual>
    


    <!-- http://purl.obolibrary.org/obo/GAZ_00598093 -->

    <owl:NamedIndividual rdf:about="http://purl.obolibrary.org/obo/GAZ_00598093">
        <obo:RO_0001025 rdf:resource="http://purl.obolibrary.org/obo/GAZ_00598087"/>
        <obo:IAO_0000115>An island.</obo:IAO_0000115>
        <oboInOwl:hasOBONamespace>GAZ</oboInOwl:hasOBONamespace>
        <oboInOwl:id>GAZ:00598093</oboInOwl:id>
        <rdfs:label>Dominikanerinsel</rdfs:label>
    </owl:NamedIndividual>
    


    <!-- http://purl.obolibrary.org/obo/GAZ_00598237 -->

    <owl:NamedIndividual rdf:about="http://purl.obolibrary.org/obo/GAZ_00598237">
        <obo:RO_0001025 rdf:resource="http://purl.obolibrary.org/obo/GAZ_00058618"/>
        <obo:IAO_0000115>A rock.</obo:IAO_0000115>
        <oboInOwl:hasOBONamespace>GAZ</oboInOwl:hasOBONamespace>
        <oboInOwl:id>GAZ:00598237</oboInOwl:id>
        <rdfs:label>Teufelstisch</rdfs:label>
    </owl:NamedIndividual>
    


    <!-- http://purl.obolibrary.org/obo/GAZ_00598326 -->

    <owl:NamedIndividual rdf:about="http://purl.obolibrary.org/obo/GAZ_00598326">
        <obo:IAO_0000115>A river.</obo:IAO_0000115>
        <oboInOwl:hasOBONamespace>GAZ</oboInOwl:hasOBONamespace>
        <oboInOwl:id>GAZ:00598326</oboInOwl:id>
        <rdfs:label>Sandwiesenbach</rdfs:label>
    </owl:NamedIndividual>
    


    <!-- http://purl.obolibrary.org/obo/GAZ_00598327 -->

    <owl:NamedIndividual rdf:about="http://purl.obolibrary.org/obo/GAZ_00598327">
        <obo:IAO_0000115>A river.</obo:IAO_0000115>
        <oboInOwl:hasOBONamespace>GAZ</oboInOwl:hasOBONamespace>
        <oboInOwl:id>GAZ:00598327</oboInOwl:id>
        <rdfs:label>Handthalergraben</rdfs:label>
    </owl:NamedIndividual>
    


    <!-- http://purl.obolibrary.org/obo/GAZ_00598328 -->

    <owl:NamedIndividual rdf:about="http://purl.obolibrary.org/obo/GAZ_00598328">
        <obo:IAO_0000115>A river.</obo:IAO_0000115>
        <oboInOwl:hasOBONamespace>GAZ</oboInOwl:hasOBONamespace>
        <oboInOwl:id>GAZ:00598328</oboInOwl:id>
        <rdfs:label>Harbach</rdfs:label>
    </owl:NamedIndividual>
    


    <!-- http://purl.obolibrary.org/obo/GAZ_00598329 -->

    <owl:NamedIndividual rdf:about="http://purl.obolibrary.org/obo/GAZ_00598329">
        <obo:IAO_0000115>A river.</obo:IAO_0000115>
        <oboInOwl:hasOBONamespace>GAZ</oboInOwl:hasOBONamespace>
        <oboInOwl:id>GAZ:00598329</oboInOwl:id>
        <rdfs:label>Schmerber Graben</rdfs:label>
    </owl:NamedIndividual>
    


    <!-- http://purl.obolibrary.org/obo/GAZ_00598330 -->

    <owl:NamedIndividual rdf:about="http://purl.obolibrary.org/obo/GAZ_00598330">
        <obo:IAO_0000115>A river.</obo:IAO_0000115>
        <oboInOwl:hasOBONamespace>GAZ</oboInOwl:hasOBONamespace>
        <oboInOwl:id>GAZ:00598330</oboInOwl:id>
        <rdfs:label>Entenbach</rdfs:label>
    </owl:NamedIndividual>
    


    <!-- http://purl.obolibrary.org/obo/GAZ_00598331 -->

    <owl:NamedIndividual rdf:about="http://purl.obolibrary.org/obo/GAZ_00598331">
        <obo:IAO_0000115>A river.</obo:IAO_0000115>
        <oboInOwl:hasOBONamespace>GAZ</oboInOwl:hasOBONamespace>
        <oboInOwl:id>GAZ:00598331</oboInOwl:id>
        <rdfs:label>Dachsgraben</rdfs:label>
    </owl:NamedIndividual>
    


    <!-- http://purl.obolibrary.org/obo/GAZ_00598332 -->

    <owl:NamedIndividual rdf:about="http://purl.obolibrary.org/obo/GAZ_00598332">
        <obo:IAO_0000115>A river.</obo:IAO_0000115>
        <oboInOwl:hasOBONamespace>GAZ</oboInOwl:hasOBONamespace>
        <oboInOwl:id>GAZ:00598332</oboInOwl:id>
        <rdfs:label>Steinachsbach</rdfs:label>
    </owl:NamedIndividual>
    


    <!-- http://purl.obolibrary.org/obo/GAZ_00598333 -->

    <owl:NamedIndividual rdf:about="http://purl.obolibrary.org/obo/GAZ_00598333">
        <obo:IAO_0000115>A river.</obo:IAO_0000115>
        <oboInOwl:hasOBONamespace>GAZ</oboInOwl:hasOBONamespace>
        <oboInOwl:id>GAZ:00598333</oboInOwl:id>
        <rdfs:label>Rambach</rdfs:label>
    </owl:NamedIndividual>
    


    <!-- http://purl.obolibrary.org/obo/GAZ_00598334 -->

    <owl:NamedIndividual rdf:about="http://purl.obolibrary.org/obo/GAZ_00598334">
        <obo:IAO_0000115>A river.</obo:IAO_0000115>
        <oboInOwl:hasOBONamespace>GAZ</oboInOwl:hasOBONamespace>
        <oboInOwl:id>GAZ:00598334</oboInOwl:id>
        <rdfs:label>Schrappachsbach</rdfs:label>
    </owl:NamedIndividual>
    


    <!-- http://purl.obolibrary.org/obo/GAZ_00598335 -->

    <owl:NamedIndividual rdf:about="http://purl.obolibrary.org/obo/GAZ_00598335">
        <obo:IAO_0000115>A river.</obo:IAO_0000115>
        <oboInOwl:hasOBONamespace>GAZ</oboInOwl:hasOBONamespace>
        <oboInOwl:id>GAZ:00598335</oboInOwl:id>
        <rdfs:label>Geiselbach</rdfs:label>
    </owl:NamedIndividual>
    


    <!-- http://purl.obolibrary.org/obo/GAZ_00598336 -->

    <owl:NamedIndividual rdf:about="http://purl.obolibrary.org/obo/GAZ_00598336">
        <obo:IAO_0000115>A river.</obo:IAO_0000115>
        <oboInOwl:hasOBONamespace>GAZ</oboInOwl:hasOBONamespace>
        <oboInOwl:id>GAZ:00598336</oboInOwl:id>
        <rdfs:label>Buchelbach</rdfs:label>
    </owl:NamedIndividual>
    


    <!-- http://purl.obolibrary.org/obo/GAZ_00598337 -->

    <owl:NamedIndividual rdf:about="http://purl.obolibrary.org/obo/GAZ_00598337">
        <obo:IAO_0000115>A river.</obo:IAO_0000115>
        <oboInOwl:hasOBONamespace>GAZ</oboInOwl:hasOBONamespace>
        <oboInOwl:id>GAZ:00598337</oboInOwl:id>
        <rdfs:label>Wolfsbach</rdfs:label>
    </owl:NamedIndividual>
    


    <!-- http://purl.obolibrary.org/obo/GAZ_00598338 -->

    <owl:NamedIndividual rdf:about="http://purl.obolibrary.org/obo/GAZ_00598338">
        <obo:IAO_0000115>A river.</obo:IAO_0000115>
        <oboInOwl:hasOBONamespace>GAZ</oboInOwl:hasOBONamespace>
        <oboInOwl:id>GAZ:00598338</oboInOwl:id>
        <rdfs:label>Dippach</rdfs:label>
    </owl:NamedIndividual>
    


    <!-- http://purl.obolibrary.org/obo/GAZ_00598339 -->

    <owl:NamedIndividual rdf:about="http://purl.obolibrary.org/obo/GAZ_00598339">
        <obo:IAO_0000115>A river.</obo:IAO_0000115>
        <oboInOwl:hasOBONamespace>GAZ</oboInOwl:hasOBONamespace>
        <oboInOwl:id>GAZ:00598339</oboInOwl:id>
        <rdfs:label>Mordersbrunnebach</rdfs:label>
    </owl:NamedIndividual>
    


    <!-- http://purl.obolibrary.org/obo/GAZ_00598340 -->

    <owl:NamedIndividual rdf:about="http://purl.obolibrary.org/obo/GAZ_00598340">
        <obo:IAO_0000115>A river.</obo:IAO_0000115>
        <oboInOwl:hasOBONamespace>GAZ</oboInOwl:hasOBONamespace>
        <oboInOwl:id>GAZ:00598340</oboInOwl:id>
        <rdfs:label>Lechgraben</rdfs:label>
    </owl:NamedIndividual>
    


    <!-- http://purl.obolibrary.org/obo/GAZ_00598341 -->

    <owl:NamedIndividual rdf:about="http://purl.obolibrary.org/obo/GAZ_00598341">
        <obo:IAO_0000115>A river.</obo:IAO_0000115>
        <oboInOwl:hasOBONamespace>GAZ</oboInOwl:hasOBONamespace>
        <oboInOwl:id>GAZ:00598341</oboInOwl:id>
        <rdfs:label>Forsdorfer Bachla</rdfs:label>
    </owl:NamedIndividual>
    


    <!-- http://purl.obolibrary.org/obo/GAZ_00599575 -->

    <owl:NamedIndividual rdf:about="http://purl.obolibrary.org/obo/GAZ_00599575">
        <obo:IAO_0000115>A river.</obo:IAO_0000115>
        <oboInOwl:hasOBONamespace>GAZ</oboInOwl:hasOBONamespace>
        <oboInOwl:id>GAZ:00599575</oboInOwl:id>
        <rdfs:label>Breitbach</rdfs:label>
    </owl:NamedIndividual>
    


    <!-- http://purl.obolibrary.org/obo/GAZ_00600495 -->

    <owl:NamedIndividual rdf:about="http://purl.obolibrary.org/obo/GAZ_00600495">
        <obo:IAO_0000115>A river.</obo:IAO_0000115>
        <oboInOwl:hasOBONamespace>GAZ</oboInOwl:hasOBONamespace>
        <oboInOwl:id>GAZ:00600495</oboInOwl:id>
        <rdfs:label>Roderbach</rdfs:label>
    </owl:NamedIndividual>
    


    <!-- http://purl.obolibrary.org/obo/GAZ_00600604 -->

    <owl:NamedIndividual rdf:about="http://purl.obolibrary.org/obo/GAZ_00600604">
        <oboInOwl:hasOBONamespace>GAZ</oboInOwl:hasOBONamespace>
        <oboInOwl:id>GAZ:00600604</oboInOwl:id>
        <rdfs:label>Neuer Graben</rdfs:label>
    </owl:NamedIndividual>
    


    <!-- http://purl.obolibrary.org/obo/GAZ_00600605 -->

    <owl:NamedIndividual rdf:about="http://purl.obolibrary.org/obo/GAZ_00600605">
        <oboInOwl:hasOBONamespace>GAZ</oboInOwl:hasOBONamespace>
        <oboInOwl:id>GAZ:00600605</oboInOwl:id>
        <rdfs:label>Hegwaldbach</rdfs:label>
    </owl:NamedIndividual>
    


    <!-- http://purl.obolibrary.org/obo/GAZ_00601488 -->

    <owl:NamedIndividual rdf:about="http://purl.obolibrary.org/obo/GAZ_00601488">
        <obo:RO_0001025 rdf:resource="http://purl.obolibrary.org/obo/GAZ_00008262"/>
        <obo:IAO_0000115>A run-of-the river hydroelectric power plant.</obo:IAO_0000115>
        <oboInOwl:hasOBONamespace>GAZ</oboInOwl:hasOBONamespace>
        <oboInOwl:id>GAZ:00601488</oboInOwl:id>
        <rdfs:label>Kraftwerk Laufenburg</rdfs:label>
    </owl:NamedIndividual>
    


    <!-- http://purl.obolibrary.org/obo/GAZ_00602608 -->

    <owl:NamedIndividual rdf:about="http://purl.obolibrary.org/obo/GAZ_00602608">
        <obo:RO_0001025 rdf:resource="http://purl.obolibrary.org/obo/GAZ_00008249"/>
        <obo:IAO_0000115>A port.</obo:IAO_0000115>
        <oboInOwl:hasOBONamespace>GAZ</oboInOwl:hasOBONamespace>
        <oboInOwl:id>GAZ:00602608</oboInOwl:id>
        <rdfs:label>Hafen Heilbronn</rdfs:label>
    </owl:NamedIndividual>
    


    <!-- http://purl.obolibrary.org/obo/GAZ_00603937 -->

    <owl:NamedIndividual rdf:about="http://purl.obolibrary.org/obo/GAZ_00603937">
        <obo:RO_0001025 rdf:resource="http://purl.obolibrary.org/obo/GAZ_00008249"/>
        <obo:IAO_0000115>A harbor.</obo:IAO_0000115>
        <oboInOwl:hasOBONamespace>GAZ</oboInOwl:hasOBONamespace>
        <oboInOwl:id>GAZ:00603937</oboInOwl:id>
        <rdfs:label>Stuttgarter Hafen</rdfs:label>
    </owl:NamedIndividual>
    


    <!-- http://purl.obolibrary.org/obo/GAZ_00605085 -->

    <owl:NamedIndividual rdf:about="http://purl.obolibrary.org/obo/GAZ_00605085">
        <obo:RO_0001025 rdf:resource="http://purl.obolibrary.org/obo/GAZ_00008249"/>
        <obo:IAO_0000115>A power station.</obo:IAO_0000115>
        <oboInOwl:hasOBONamespace>GAZ</oboInOwl:hasOBONamespace>
        <oboInOwl:id>GAZ:00605085</oboInOwl:id>
        <rdfs:label>Wasserkraftwerk Bad Niedernau</rdfs:label>
    </owl:NamedIndividual>
    


    <!-- http://purl.obolibrary.org/obo/GAZ_00605086 -->

    <owl:NamedIndividual rdf:about="http://purl.obolibrary.org/obo/GAZ_00605086">
        <obo:RO_0001025 rdf:resource="http://purl.obolibrary.org/obo/GAZ_00008249"/>
        <obo:IAO_0000115>A power station.</obo:IAO_0000115>
        <oboInOwl:hasOBONamespace>GAZ</oboInOwl:hasOBONamespace>
        <oboInOwl:id>GAZ:00605086</oboInOwl:id>
        <rdfs:label>Wasserkraftwerk Kiebingen</rdfs:label>
    </owl:NamedIndividual>
    


    <!-- http://purl.obolibrary.org/obo/GAZ_00605087 -->

    <owl:NamedIndividual rdf:about="http://purl.obolibrary.org/obo/GAZ_00605087">
        <obo:RO_0001025 rdf:resource="http://purl.obolibrary.org/obo/GAZ_00008249"/>
        <obo:IAO_0000115>A power station.</obo:IAO_0000115>
        <oboInOwl:hasOBONamespace>GAZ</oboInOwl:hasOBONamespace>
        <oboInOwl:id>GAZ:00605087</oboInOwl:id>
        <rdfs:label>Flusskraftwerk Tubinger Strasse</rdfs:label>
    </owl:NamedIndividual>
    


    <!-- http://purl.obolibrary.org/obo/GAZ_00605088 -->

    <owl:NamedIndividual rdf:about="http://purl.obolibrary.org/obo/GAZ_00605088">
        <obo:RO_0001025 rdf:resource="http://purl.obolibrary.org/obo/GAZ_00008249"/>
        <obo:IAO_0000115>A power station.</obo:IAO_0000115>
        <oboInOwl:hasOBONamespace>GAZ</oboInOwl:hasOBONamespace>
        <oboInOwl:id>GAZ:00605088</oboInOwl:id>
        <rdfs:label>Flusskraftwerk Beim Preussischen</rdfs:label>
    </owl:NamedIndividual>
    


    <!-- http://purl.obolibrary.org/obo/GAZ_00605220 -->

    <owl:NamedIndividual rdf:about="http://purl.obolibrary.org/obo/GAZ_00605220">
        <obo:IAO_0000115>A flood-control reservoir.</obo:IAO_0000115>
        <oboInOwl:hasOBONamespace>GAZ</oboInOwl:hasOBONamespace>
        <oboInOwl:id>GAZ:00605220</oboInOwl:id>
        <rdfs:label>Hochwasserruckhaltebecken Segelbach</rdfs:label>
    </owl:NamedIndividual>
    


    <!-- http://purl.obolibrary.org/obo/GAZ_00605248 -->

    <owl:NamedIndividual rdf:about="http://purl.obolibrary.org/obo/GAZ_00605248">
        <obo:IAO_0000115>A river.</obo:IAO_0000115>
        <oboInOwl:hasOBONamespace>GAZ</oboInOwl:hasOBONamespace>
        <oboInOwl:id>GAZ:00605248</oboInOwl:id>
        <rdfs:label>Herdenbach</rdfs:label>
    </owl:NamedIndividual>
    


    <!-- http://purl.obolibrary.org/obo/GAZ_00605249 -->

    <owl:NamedIndividual rdf:about="http://purl.obolibrary.org/obo/GAZ_00605249">
        <obo:IAO_0000115>A river.</obo:IAO_0000115>
        <oboInOwl:hasOBONamespace>GAZ</oboInOwl:hasOBONamespace>
        <oboInOwl:id>GAZ:00605249</oboInOwl:id>
        <rdfs:label>Waschbach</rdfs:label>
    </owl:NamedIndividual>
    


    <!-- http://purl.obolibrary.org/obo/GAZ_00605250 -->

    <owl:NamedIndividual rdf:about="http://purl.obolibrary.org/obo/GAZ_00605250">
        <obo:IAO_0000115>A river.</obo:IAO_0000115>
        <oboInOwl:hasOBONamespace>GAZ</oboInOwl:hasOBONamespace>
        <oboInOwl:id>GAZ:00605250</oboInOwl:id>
        <rdfs:label>Torpenbach</rdfs:label>
    </owl:NamedIndividual>
    


    <!-- http://purl.obolibrary.org/obo/GAZ_00605251 -->

    <owl:NamedIndividual rdf:about="http://purl.obolibrary.org/obo/GAZ_00605251">
        <obo:IAO_0000115>A river.</obo:IAO_0000115>
        <oboInOwl:hasOBONamespace>GAZ</oboInOwl:hasOBONamespace>
        <oboInOwl:id>GAZ:00605251</oboInOwl:id>
        <rdfs:label>Nellenflurbach</rdfs:label>
    </owl:NamedIndividual>
    


    <!-- http://purl.obolibrary.org/obo/GAZ_00605252 -->

    <owl:NamedIndividual rdf:about="http://purl.obolibrary.org/obo/GAZ_00605252">
        <obo:IAO_0000115>A river.</obo:IAO_0000115>
        <oboInOwl:hasOBONamespace>GAZ</oboInOwl:hasOBONamespace>
        <oboInOwl:id>GAZ:00605252</oboInOwl:id>
        <rdfs:label>Furtbach</rdfs:label>
    </owl:NamedIndividual>
    


    <!-- http://purl.obolibrary.org/obo/GAZ_00605253 -->

    <owl:NamedIndividual rdf:about="http://purl.obolibrary.org/obo/GAZ_00605253">
        <obo:IAO_0000115>A river.</obo:IAO_0000115>
        <oboInOwl:hasOBONamespace>GAZ</oboInOwl:hasOBONamespace>
        <oboInOwl:id>GAZ:00605253</oboInOwl:id>
        <rdfs:label>Erlengraben</rdfs:label>
    </owl:NamedIndividual>
    


    <!-- http://purl.obolibrary.org/obo/GAZ_00605254 -->

    <owl:NamedIndividual rdf:about="http://purl.obolibrary.org/obo/GAZ_00605254">
        <obo:IAO_0000115>A river.</obo:IAO_0000115>
        <oboInOwl:hasOBONamespace>GAZ</oboInOwl:hasOBONamespace>
        <oboInOwl:id>GAZ:00605254</oboInOwl:id>
        <rdfs:label>Aubach</rdfs:label>
    </owl:NamedIndividual>
    


    <!-- http://purl.obolibrary.org/obo/GAZ_00605255 -->

    <owl:NamedIndividual rdf:about="http://purl.obolibrary.org/obo/GAZ_00605255">
        <obo:IAO_0000115>A river.</obo:IAO_0000115>
        <oboInOwl:hasOBONamespace>GAZ</oboInOwl:hasOBONamespace>
        <oboInOwl:id>GAZ:00605255</oboInOwl:id>
        <rdfs:label>Deggenhauser Aach</rdfs:label>
    </owl:NamedIndividual>
    


    <!-- http://purl.obolibrary.org/obo/GAZ_00605256 -->

    <owl:NamedIndividual rdf:about="http://purl.obolibrary.org/obo/GAZ_00605256">
        <obo:IAO_0000115>A river.</obo:IAO_0000115>
        <oboInOwl:hasOBONamespace>GAZ</oboInOwl:hasOBONamespace>
        <oboInOwl:id>GAZ:00605256</oboInOwl:id>
        <rdfs:label>Giessbach</rdfs:label>
    </owl:NamedIndividual>
    


    <!-- http://purl.obolibrary.org/obo/GAZ_00605257 -->

    <owl:NamedIndividual rdf:about="http://purl.obolibrary.org/obo/GAZ_00605257">
        <obo:IAO_0000115>A river.</obo:IAO_0000115>
        <oboInOwl:hasOBONamespace>GAZ</oboInOwl:hasOBONamespace>
        <oboInOwl:id>GAZ:00605257</oboInOwl:id>
        <rdfs:label>Lautenbach</rdfs:label>
    </owl:NamedIndividual>
    


    <!-- http://purl.obolibrary.org/obo/GAZ_00605321 -->

    <owl:NamedIndividual rdf:about="http://purl.obolibrary.org/obo/GAZ_00605321">
        <obo:IAO_0000115>A reservoir.</obo:IAO_0000115>
        <oboInOwl:hasOBONamespace>GAZ</oboInOwl:hasOBONamespace>
        <oboInOwl:id>GAZ:00605321</oboInOwl:id>
        <rdfs:label>Ehmetsklinge</rdfs:label>
    </owl:NamedIndividual>
    


    <!-- http://purl.obolibrary.org/obo/GAZ_00605556 -->

    <owl:NamedIndividual rdf:about="http://purl.obolibrary.org/obo/GAZ_00605556">
        <obo:IAO_0000115>A river.</obo:IAO_0000115>
        <oboInOwl:hasOBONamespace>GAZ</oboInOwl:hasOBONamespace>
        <oboInOwl:id>GAZ:00605556</oboInOwl:id>
        <rdfs:label>Seebach</rdfs:label>
    </owl:NamedIndividual>
    


    <!-- http://purl.obolibrary.org/obo/GAZ_00605557 -->

    <owl:NamedIndividual rdf:about="http://purl.obolibrary.org/obo/GAZ_00605557">
        <obo:IAO_0000115>A river.</obo:IAO_0000115>
        <oboInOwl:hasOBONamespace>GAZ</oboInOwl:hasOBONamespace>
        <oboInOwl:id>GAZ:00605557</oboInOwl:id>
        <rdfs:label>Grimmerswaldbach</rdfs:label>
    </owl:NamedIndividual>
    


    <!-- http://purl.obolibrary.org/obo/GAZ_00605558 -->

    <owl:NamedIndividual rdf:about="http://purl.obolibrary.org/obo/GAZ_00605558">
        <obo:IAO_0000115>A river.</obo:IAO_0000115>
        <oboInOwl:hasOBONamespace>GAZ</oboInOwl:hasOBONamespace>
        <oboInOwl:id>GAZ:00605558</oboInOwl:id>
        <rdfs:label>Sulzbach</rdfs:label>
    </owl:NamedIndividual>
    


    <!-- http://purl.obolibrary.org/obo/GAZ_00605559 -->

    <owl:NamedIndividual rdf:about="http://purl.obolibrary.org/obo/GAZ_00605559">
        <obo:IAO_0000115>A river.</obo:IAO_0000115>
        <oboInOwl:hasOBONamespace>GAZ</oboInOwl:hasOBONamespace>
        <oboInOwl:id>GAZ:00605559</oboInOwl:id>
        <rdfs:label>Sandbach</rdfs:label>
    </owl:NamedIndividual>
    


    <!-- http://purl.obolibrary.org/obo/GAZ_00605560 -->

    <owl:NamedIndividual rdf:about="http://purl.obolibrary.org/obo/GAZ_00605560">
        <obo:IAO_0000115>A river.</obo:IAO_0000115>
        <oboInOwl:hasOBONamespace>GAZ</oboInOwl:hasOBONamespace>
        <oboInOwl:id>GAZ:00605560</oboInOwl:id>
        <rdfs:label>Gottschlagbach</rdfs:label>
    </owl:NamedIndividual>
    


    <!-- http://purl.obolibrary.org/obo/GAZ_00605561 -->

    <owl:NamedIndividual rdf:about="http://purl.obolibrary.org/obo/GAZ_00605561">
        <obo:IAO_0000115>A river.</obo:IAO_0000115>
        <oboInOwl:hasOBONamespace>GAZ</oboInOwl:hasOBONamespace>
        <oboInOwl:id>GAZ:00605561</oboInOwl:id>
        <rdfs:label>Unterwasserbach</rdfs:label>
    </owl:NamedIndividual>
    


    <!-- http://purl.obolibrary.org/obo/GAZ_00605562 -->

    <owl:NamedIndividual rdf:about="http://purl.obolibrary.org/obo/GAZ_00605562">
        <obo:IAO_0000115>A river.</obo:IAO_0000115>
        <oboInOwl:hasOBONamespace>GAZ</oboInOwl:hasOBONamespace>
        <oboInOwl:id>GAZ:00605562</oboInOwl:id>
        <rdfs:label>Fautenbach</rdfs:label>
    </owl:NamedIndividual>
    


    <!-- http://purl.obolibrary.org/obo/GAZ_00606252 -->

    <owl:NamedIndividual rdf:about="http://purl.obolibrary.org/obo/GAZ_00606252">
        <obo:IAO_0000115>A river.</obo:IAO_0000115>
        <oboInOwl:hasOBONamespace>GAZ</oboInOwl:hasOBONamespace>
        <oboInOwl:id>GAZ:00606252</oboInOwl:id>
        <rdfs:label>Klapperschenkelbach</rdfs:label>
    </owl:NamedIndividual>
    


    <!-- http://purl.obolibrary.org/obo/GAZ_00606253 -->

    <owl:NamedIndividual rdf:about="http://purl.obolibrary.org/obo/GAZ_00606253">
        <obo:IAO_0000115>A river.</obo:IAO_0000115>
        <oboInOwl:hasOBONamespace>GAZ</oboInOwl:hasOBONamespace>
        <oboInOwl:id>GAZ:00606253</oboInOwl:id>
        <rdfs:label>Gallenfeldbach</rdfs:label>
    </owl:NamedIndividual>
    


    <!-- http://purl.obolibrary.org/obo/GAZ_00606254 -->

    <owl:NamedIndividual rdf:about="http://purl.obolibrary.org/obo/GAZ_00606254">
        <obo:IAO_0000115>A river.</obo:IAO_0000115>
        <oboInOwl:hasOBONamespace>GAZ</oboInOwl:hasOBONamespace>
        <oboInOwl:id>GAZ:00606254</oboInOwl:id>
        <rdfs:label>Sagbach</rdfs:label>
    </owl:NamedIndividual>
    


    <!-- http://purl.obolibrary.org/obo/GAZ_00606255 -->

    <owl:NamedIndividual rdf:about="http://purl.obolibrary.org/obo/GAZ_00606255">
        <obo:IAO_0000115>A river.</obo:IAO_0000115>
        <oboInOwl:hasOBONamespace>GAZ</oboInOwl:hasOBONamespace>
        <oboInOwl:id>GAZ:00606255</oboInOwl:id>
        <rdfs:label>Lindenhofbach</rdfs:label>
    </owl:NamedIndividual>
    


    <!-- http://purl.obolibrary.org/obo/GAZ_00606256 -->

    <owl:NamedIndividual rdf:about="http://purl.obolibrary.org/obo/GAZ_00606256">
        <obo:IAO_0000115>A river.</obo:IAO_0000115>
        <oboInOwl:hasOBONamespace>GAZ</oboInOwl:hasOBONamespace>
        <oboInOwl:id>GAZ:00606256</oboInOwl:id>
        <rdfs:label>Beerenholzlebach</rdfs:label>
    </owl:NamedIndividual>
    


    <!-- http://purl.obolibrary.org/obo/GAZ_00606257 -->

    <owl:NamedIndividual rdf:about="http://purl.obolibrary.org/obo/GAZ_00606257">
        <obo:IAO_0000115>A river.</obo:IAO_0000115>
        <oboInOwl:hasOBONamespace>GAZ</oboInOwl:hasOBONamespace>
        <oboInOwl:id>GAZ:00606257</oboInOwl:id>
        <rdfs:label>Hinterbrandbach</rdfs:label>
    </owl:NamedIndividual>
    


    <!-- http://purl.obolibrary.org/obo/GAZ_00606258 -->

    <owl:NamedIndividual rdf:about="http://purl.obolibrary.org/obo/GAZ_00606258">
        <obo:IAO_0000115>A river.</obo:IAO_0000115>
        <oboInOwl:hasOBONamespace>GAZ</oboInOwl:hasOBONamespace>
        <oboInOwl:id>GAZ:00606258</oboInOwl:id>
        <rdfs:label>Herzbuhlbach</rdfs:label>
    </owl:NamedIndividual>
    


    <!-- http://purl.obolibrary.org/obo/GAZ_00606259 -->

    <owl:NamedIndividual rdf:about="http://purl.obolibrary.org/obo/GAZ_00606259">
        <obo:IAO_0000115>A river.</obo:IAO_0000115>
        <oboInOwl:hasOBONamespace>GAZ</oboInOwl:hasOBONamespace>
        <oboInOwl:id>GAZ:00606259</oboInOwl:id>
        <rdfs:label>Wolfsbach</rdfs:label>
    </owl:NamedIndividual>
    


    <!-- http://purl.obolibrary.org/obo/GAZ_00606260 -->

    <owl:NamedIndividual rdf:about="http://purl.obolibrary.org/obo/GAZ_00606260">
        <obo:IAO_0000115>A river.</obo:IAO_0000115>
        <oboInOwl:hasOBONamespace>GAZ</oboInOwl:hasOBONamespace>
        <oboInOwl:id>GAZ:00606260</oboInOwl:id>
        <rdfs:label>Hohlspitzbach</rdfs:label>
    </owl:NamedIndividual>
    


    <!-- http://purl.obolibrary.org/obo/GAZ_00606261 -->

    <owl:NamedIndividual rdf:about="http://purl.obolibrary.org/obo/GAZ_00606261">
        <obo:IAO_0000115>A river.</obo:IAO_0000115>
        <oboInOwl:hasOBONamespace>GAZ</oboInOwl:hasOBONamespace>
        <oboInOwl:id>GAZ:00606261</oboInOwl:id>
        <rdfs:label>Kaltenbach</rdfs:label>
    </owl:NamedIndividual>
    


    <!-- http://purl.obolibrary.org/obo/GAZ_00606262 -->

    <owl:NamedIndividual rdf:about="http://purl.obolibrary.org/obo/GAZ_00606262">
        <obo:IAO_0000115>A river.</obo:IAO_0000115>
        <oboInOwl:hasOBONamespace>GAZ</oboInOwl:hasOBONamespace>
        <oboInOwl:id>GAZ:00606262</oboInOwl:id>
        <rdfs:label>Entenbach</rdfs:label>
    </owl:NamedIndividual>
    


    <!-- http://purl.obolibrary.org/obo/GAZ_00606263 -->

    <owl:NamedIndividual rdf:about="http://purl.obolibrary.org/obo/GAZ_00606263">
        <obo:IAO_0000115>A river.</obo:IAO_0000115>
        <oboInOwl:hasOBONamespace>GAZ</oboInOwl:hasOBONamespace>
        <oboInOwl:id>GAZ:00606263</oboInOwl:id>
        <rdfs:label>Sekretarsbach</rdfs:label>
    </owl:NamedIndividual>
    


    <!-- http://purl.obolibrary.org/obo/GAZ_00606264 -->

    <owl:NamedIndividual rdf:about="http://purl.obolibrary.org/obo/GAZ_00606264">
        <obo:IAO_0000115>A river.</obo:IAO_0000115>
        <oboInOwl:hasOBONamespace>GAZ</oboInOwl:hasOBONamespace>
        <oboInOwl:id>GAZ:00606264</oboInOwl:id>
        <rdfs:label>Gabelbach</rdfs:label>
    </owl:NamedIndividual>
    


    <!-- http://purl.obolibrary.org/obo/GAZ_00606270 -->

    <owl:NamedIndividual rdf:about="http://purl.obolibrary.org/obo/GAZ_00606270">
        <obo:IAO_0000115>A reservoir.</obo:IAO_0000115>
        <oboInOwl:hasOBONamespace>GAZ</oboInOwl:hasOBONamespace>
        <oboInOwl:id>GAZ:00606270</oboInOwl:id>
        <rdfs:label>Ausgleichsbecken Forbach</rdfs:label>
    </owl:NamedIndividual>
    


    <!-- http://purl.obolibrary.org/obo/GAZ_00606280 -->

    <owl:NamedIndividual rdf:about="http://purl.obolibrary.org/obo/GAZ_00606280">
        <obo:IAO_0000115>A reservoir.</obo:IAO_0000115>
        <oboInOwl:hasOBONamespace>GAZ</oboInOwl:hasOBONamespace>
        <oboInOwl:id>GAZ:00606280</oboInOwl:id>
        <rdfs:label>Murgtalsperre Kirschbaumwasen</rdfs:label>
    </owl:NamedIndividual>
    


    <!-- http://purl.obolibrary.org/obo/GAZ_00606455 -->

    <owl:NamedIndividual rdf:about="http://purl.obolibrary.org/obo/GAZ_00606455">
        <obo:IAO_0000115>A river.</obo:IAO_0000115>
        <oboInOwl:hasOBONamespace>GAZ</oboInOwl:hasOBONamespace>
        <oboInOwl:id>GAZ:00606455</oboInOwl:id>
        <rdfs:label>Tannenbach</rdfs:label>
    </owl:NamedIndividual>
    


    <!-- http://purl.obolibrary.org/obo/GAZ_00606468 -->

    <owl:NamedIndividual rdf:about="http://purl.obolibrary.org/obo/GAZ_00606468">
        <obo:IAO_0000115>A lake.</obo:IAO_0000115>
        <oboInOwl:hasOBONamespace>GAZ</oboInOwl:hasOBONamespace>
        <oboInOwl:id>GAZ:00606468</oboInOwl:id>
        <rdfs:label>Bombensee</rdfs:label>
    </owl:NamedIndividual>
    


    <!-- http://purl.obolibrary.org/obo/GAZ_00606671 -->

    <owl:NamedIndividual rdf:about="http://purl.obolibrary.org/obo/GAZ_00606671">
        <obo:IAO_0000115>A pumped-station reservoir.</obo:IAO_0000115>
        <oboInOwl:hasOBONamespace>GAZ</oboInOwl:hasOBONamespace>
        <oboInOwl:id>GAZ:00606671</oboInOwl:id>
        <rdfs:label>Mettmastausee</rdfs:label>
    </owl:NamedIndividual>
    


    <!-- http://purl.obolibrary.org/obo/GAZ_00606676 -->

    <owl:NamedIndividual rdf:about="http://purl.obolibrary.org/obo/GAZ_00606676">
        <obo:IAO_0000115>A reservoir and dam.</obo:IAO_0000115>
        <oboInOwl:hasOBONamespace>GAZ</oboInOwl:hasOBONamespace>
        <oboInOwl:id>GAZ:00606676</oboInOwl:id>
        <rdfs:label>Wehratalsperre</rdfs:label>
    </owl:NamedIndividual>
    


    <!-- http://purl.obolibrary.org/obo/GAZ_00606683 -->

    <owl:NamedIndividual rdf:about="http://purl.obolibrary.org/obo/GAZ_00606683">
        <obo:IAO_0000115>A reservoir.</obo:IAO_0000115>
        <oboInOwl:hasOBONamespace>GAZ</oboInOwl:hasOBONamespace>
        <oboInOwl:id>GAZ:00606683</oboInOwl:id>
        <rdfs:label>Schlichemtalsperre</rdfs:label>
    </owl:NamedIndividual>
    


    <!-- http://purl.obolibrary.org/obo/GAZ_00606766 -->

    <owl:NamedIndividual rdf:about="http://purl.obolibrary.org/obo/GAZ_00606766">
        <obo:RO_0001025 rdf:resource="http://purl.obolibrary.org/obo/GAZ_00008262"/>
        <obo:IAO_0000115>A man-made fluvial island in the Rhine.</obo:IAO_0000115>
        <oboInOwl:hasOBONamespace>GAZ</oboInOwl:hasOBONamespace>
        <oboInOwl:id>GAZ:00606766</oboInOwl:id>
        <rdfs:label>Elisabethenworth</rdfs:label>
    </owl:NamedIndividual>
    


    <!-- http://purl.obolibrary.org/obo/GAZ_00606767 -->

    <owl:NamedIndividual rdf:about="http://purl.obolibrary.org/obo/GAZ_00606767">
        <rdf:type rdf:resource="http://purl.obolibrary.org/obo/ENVO_00000423"/>
        <obo:RO_0001025 rdf:resource="http://purl.obolibrary.org/obo/GAZ_00008262"/>
        <obo:IAO_0000115>A fluvial island that developed after the construction of the Bad Sackingen power station. Ownership (German (Bad Sackingen) or Swiss (Stein)) not clear.</obo:IAO_0000115>
        <oboInOwl:hasOBONamespace>GAZ</oboInOwl:hasOBONamespace>
        <oboInOwl:id>GAZ:00606767</oboInOwl:id>
        <rdfs:label>Fridolininsel</rdfs:label>
    </owl:NamedIndividual>
    


    <!-- http://purl.obolibrary.org/obo/GAZ_00606768 -->

    <owl:NamedIndividual rdf:about="http://purl.obolibrary.org/obo/GAZ_00606768">
        <rdf:type rdf:resource="http://purl.obolibrary.org/obo/ENVO_00000423"/>
        <obo:RO_0001025 rdf:resource="http://purl.obolibrary.org/obo/GAZ_00008262"/>
        <obo:IAO_0000115>A fluvial island.</obo:IAO_0000115>
        <oboInOwl:hasOBONamespace>GAZ</oboInOwl:hasOBONamespace>
        <oboInOwl:id>GAZ:00606768</oboInOwl:id>
        <rdfs:label>Judenaule</rdfs:label>
    </owl:NamedIndividual>
    


    <!-- http://purl.obolibrary.org/obo/GAZ_00606823 -->

    <owl:NamedIndividual rdf:about="http://purl.obolibrary.org/obo/GAZ_00606823">
        <obo:IAO_0000115>A river.</obo:IAO_0000115>
        <oboInOwl:hasOBONamespace>GAZ</oboInOwl:hasOBONamespace>
        <oboInOwl:id>GAZ:00606823</oboInOwl:id>
        <rdfs:label>Gygerbachli bei Walde</rdfs:label>
    </owl:NamedIndividual>
    


    <!-- http://purl.obolibrary.org/obo/GAZ_00606824 -->

    <owl:NamedIndividual rdf:about="http://purl.obolibrary.org/obo/GAZ_00606824">
        <obo:IAO_0000115>A river.</obo:IAO_0000115>
        <oboInOwl:hasOBONamespace>GAZ</oboInOwl:hasOBONamespace>
        <oboInOwl:id>GAZ:00606824</oboInOwl:id>
        <rdfs:label>Lorentobe</rdfs:label>
    </owl:NamedIndividual>
    


    <!-- http://purl.obolibrary.org/obo/GAZ_00606825 -->

    <owl:NamedIndividual rdf:about="http://purl.obolibrary.org/obo/GAZ_00606825">
        <obo:IAO_0000115>A river.</obo:IAO_0000115>
        <oboInOwl:hasOBONamespace>GAZ</oboInOwl:hasOBONamespace>
        <oboInOwl:id>GAZ:00606825</oboInOwl:id>
        <rdfs:label>Anzigraben</rdfs:label>
    </owl:NamedIndividual>
    


    <!-- http://purl.obolibrary.org/obo/GAZ_00606826 -->

    <owl:NamedIndividual rdf:about="http://purl.obolibrary.org/obo/GAZ_00606826">
        <obo:IAO_0000115>A river.</obo:IAO_0000115>
        <oboInOwl:hasOBONamespace>GAZ</oboInOwl:hasOBONamespace>
        <oboInOwl:id>GAZ:00606826</oboInOwl:id>
        <rdfs:label>Steinigbach</rdfs:label>
    </owl:NamedIndividual>
    


    <!-- http://purl.obolibrary.org/obo/GAZ_00606827 -->

    <owl:NamedIndividual rdf:about="http://purl.obolibrary.org/obo/GAZ_00606827">
        <obo:IAO_0000115>A river.</obo:IAO_0000115>
        <oboInOwl:hasOBONamespace>GAZ</oboInOwl:hasOBONamespace>
        <oboInOwl:id>GAZ:00606827</oboInOwl:id>
        <rdfs:label>Bach von Hasel</rdfs:label>
    </owl:NamedIndividual>
    


    <!-- http://purl.obolibrary.org/obo/GAZ_00607595 -->

    <owl:NamedIndividual rdf:about="http://purl.obolibrary.org/obo/GAZ_00607595">
        <obo:IAO_0000115>A lake; located on Staatsstrasse 2019 (Krumbach - Weissenhorn) between Deisenhausen and Ingstetten.</obo:IAO_0000115>
        <oboInOwl:hasOBONamespace>GAZ</oboInOwl:hasOBONamespace>
        <oboInOwl:id>GAZ:00607595</oboInOwl:id>
        <rdfs:label>Ingstetter Weiher</rdfs:label>
    </owl:NamedIndividual>
    


    <!-- http://purl.obolibrary.org/obo/GAZ_00607669 -->

    <owl:NamedIndividual rdf:about="http://purl.obolibrary.org/obo/GAZ_00607669">
        <obo:RO_0001025 rdf:resource="http://purl.obolibrary.org/obo/GAZ_00060652"/>
        <obo:IAO_0000115>A lake.</obo:IAO_0000115>
        <oboInOwl:hasOBONamespace>GAZ</oboInOwl:hasOBONamespace>
        <oboInOwl:id>GAZ:00607669</oboInOwl:id>
        <rdfs:label>Kochelsee</rdfs:label>
    </owl:NamedIndividual>
    


    <!-- http://purl.obolibrary.org/obo/GAZ_00609318 -->

    <owl:NamedIndividual rdf:about="http://purl.obolibrary.org/obo/GAZ_00609318">
        <obo:RO_0001025 rdf:resource="http://purl.obolibrary.org/obo/GAZ_00060655"/>
        <obo:IAO_0000115>A lacustrine island.</obo:IAO_0000115>
        <oboInOwl:hasOBONamespace>GAZ</oboInOwl:hasOBONamespace>
        <oboInOwl:id>GAZ:00609318</oboInOwl:id>
        <rdfs:label>Ringsee-Insel</rdfs:label>
    </owl:NamedIndividual>
    


    <!-- http://purl.obolibrary.org/obo/GAZ_00609567 -->

    <owl:NamedIndividual rdf:about="http://purl.obolibrary.org/obo/GAZ_00609567">
        <obo:RO_0001025 rdf:resource="http://purl.obolibrary.org/obo/GAZ_00607669"/>
        <obo:IAO_0000115>A hydroelectric power station.</obo:IAO_0000115>
        <oboInOwl:hasOBONamespace>GAZ</oboInOwl:hasOBONamespace>
        <oboInOwl:id>GAZ:00609567</oboInOwl:id>
        <rdfs:label>Walchenseekraftwerk</rdfs:label>
    </owl:NamedIndividual>
    


    <!-- http://purl.obolibrary.org/obo/GAZ_00609874 -->

    <owl:NamedIndividual rdf:about="http://purl.obolibrary.org/obo/GAZ_00609874">
        <obo:IAO_0000115>A river.</obo:IAO_0000115>
        <oboInOwl:hasOBONamespace>GAZ</oboInOwl:hasOBONamespace>
        <oboInOwl:id>GAZ:00609874</oboInOwl:id>
        <rdfs:label>Wildwurmgraben</rdfs:label>
    </owl:NamedIndividual>
    


    <!-- http://purl.obolibrary.org/obo/GAZ_00609875 -->

    <owl:NamedIndividual rdf:about="http://purl.obolibrary.org/obo/GAZ_00609875">
        <obo:IAO_0000115>A river.</obo:IAO_0000115>
        <oboInOwl:hasOBONamespace>GAZ</oboInOwl:hasOBONamespace>
        <oboInOwl:id>GAZ:00609875</oboInOwl:id>
        <rdfs:label>Steingraben</rdfs:label>
    </owl:NamedIndividual>
    


    <!-- http://purl.obolibrary.org/obo/GAZ_00609876 -->

    <owl:NamedIndividual rdf:about="http://purl.obolibrary.org/obo/GAZ_00609876">
        <obo:IAO_0000115>A river.</obo:IAO_0000115>
        <oboInOwl:hasOBONamespace>GAZ</oboInOwl:hasOBONamespace>
        <oboInOwl:id>GAZ:00609876</oboInOwl:id>
        <rdfs:label>Schlossgraben</rdfs:label>
    </owl:NamedIndividual>
    


    <!-- http://purl.obolibrary.org/obo/GAZ_00609877 -->

    <owl:NamedIndividual rdf:about="http://purl.obolibrary.org/obo/GAZ_00609877">
        <obo:IAO_0000115>A river.</obo:IAO_0000115>
        <oboInOwl:hasOBONamespace>GAZ</oboInOwl:hasOBONamespace>
        <oboInOwl:id>GAZ:00609877</oboInOwl:id>
        <rdfs:label>Eichgraben</rdfs:label>
    </owl:NamedIndividual>
    


    <!-- http://purl.obolibrary.org/obo/GAZ_00611386 -->

    <owl:NamedIndividual rdf:about="http://purl.obolibrary.org/obo/GAZ_00611386">
        <obo:IAO_0000115>A reservoir.</obo:IAO_0000115>
        <oboInOwl:hasOBONamespace>GAZ</oboInOwl:hasOBONamespace>
        <oboInOwl:id>GAZ:00611386</oboInOwl:id>
        <rdfs:label>Stausee am Asbach</rdfs:label>
    </owl:NamedIndividual>
    


    <!-- http://purl.obolibrary.org/obo/GAZ_00612221 -->

    <owl:NamedIndividual rdf:about="http://purl.obolibrary.org/obo/GAZ_00612221">
        <obo:IAO_0000115>A former canal. It linked the Danube River at Kelheim with the Main River at Bamberg, connecting the Danube basin with the Rhine basin.</obo:IAO_0000115>
        <oboInOwl:hasOBONamespace>GAZ</oboInOwl:hasOBONamespace>
        <oboInOwl:id>GAZ:00612221</oboInOwl:id>
        <rdfs:label>Ludwig-Donau-Main-Kanal</rdfs:label>
    </owl:NamedIndividual>
    


    <!-- http://purl.obolibrary.org/obo/GAZ_00612272 -->

    <owl:NamedIndividual rdf:about="http://purl.obolibrary.org/obo/GAZ_00612272">
        <obo:IAO_0000115>A lock.</obo:IAO_0000115>
        <oboInOwl:hasOBONamespace>GAZ</oboInOwl:hasOBONamespace>
        <oboInOwl:id>GAZ:00612272</oboInOwl:id>
        <rdfs:label>Schleuse Leerstetten</rdfs:label>
    </owl:NamedIndividual>
    


    <!-- http://purl.obolibrary.org/obo/GAZ_00612914 -->

    <owl:NamedIndividual rdf:about="http://purl.obolibrary.org/obo/GAZ_00612914">
        <obo:IAO_0000115>A river.</obo:IAO_0000115>
        <oboInOwl:hasOBONamespace>GAZ</oboInOwl:hasOBONamespace>
        <oboInOwl:id>GAZ:00612914</oboInOwl:id>
        <rdfs:label>Anifer Alterbach</rdfs:label>
    </owl:NamedIndividual>
    


    <!-- http://purl.obolibrary.org/obo/GAZ_00612959 -->

    <owl:NamedIndividual rdf:about="http://purl.obolibrary.org/obo/GAZ_00612959">
        <obo:IAO_0000115>A river.</obo:IAO_0000115>
        <oboInOwl:hasOBONamespace>GAZ</oboInOwl:hasOBONamespace>
        <oboInOwl:id>GAZ:00612959</oboInOwl:id>
        <rdfs:label>Kleine Isar</rdfs:label>
    </owl:NamedIndividual>
    


    <!-- http://purl.obolibrary.org/obo/GAZ_00612967 -->

    <owl:NamedIndividual rdf:about="http://purl.obolibrary.org/obo/GAZ_00612967">
        <obo:IAO_0000115>A river.</obo:IAO_0000115>
        <oboInOwl:hasOBONamespace>GAZ</oboInOwl:hasOBONamespace>
        <oboInOwl:id>GAZ:00612967</oboInOwl:id>
        <rdfs:label>Weissenbach</rdfs:label>
    </owl:NamedIndividual>
    


    <!-- http://purl.obolibrary.org/obo/GAZ_00612968 -->

    <owl:NamedIndividual rdf:about="http://purl.obolibrary.org/obo/GAZ_00612968">
        <obo:IAO_0000115>A river.</obo:IAO_0000115>
        <oboInOwl:hasOBONamespace>GAZ</oboInOwl:hasOBONamespace>
        <oboInOwl:id>GAZ:00612968</oboInOwl:id>
        <rdfs:label>Bayerbach</rdfs:label>
    </owl:NamedIndividual>
    


    <!-- http://purl.obolibrary.org/obo/GAZ_00612969 -->

    <owl:NamedIndividual rdf:about="http://purl.obolibrary.org/obo/GAZ_00612969">
        <obo:IAO_0000115>A river.</obo:IAO_0000115>
        <oboInOwl:hasOBONamespace>GAZ</oboInOwl:hasOBONamespace>
        <oboInOwl:id>GAZ:00612969</oboInOwl:id>
        <rdfs:label>Hengstbach</rdfs:label>
    </owl:NamedIndividual>
    


    <!-- http://purl.obolibrary.org/obo/GAZ_00612970 -->

    <owl:NamedIndividual rdf:about="http://purl.obolibrary.org/obo/GAZ_00612970">
        <obo:IAO_0000115>A river.</obo:IAO_0000115>
        <oboInOwl:hasOBONamespace>GAZ</oboInOwl:hasOBONamespace>
        <oboInOwl:id>GAZ:00612970</oboInOwl:id>
        <rdfs:label>Rehgraben</rdfs:label>
    </owl:NamedIndividual>
    


    <!-- http://purl.obolibrary.org/obo/GAZ_00612971 -->

    <owl:NamedIndividual rdf:about="http://purl.obolibrary.org/obo/GAZ_00612971">
        <obo:IAO_0000115>A river.</obo:IAO_0000115>
        <oboInOwl:hasOBONamespace>GAZ</oboInOwl:hasOBONamespace>
        <oboInOwl:id>GAZ:00612971</oboInOwl:id>
        <rdfs:label>Kohlgraben</rdfs:label>
    </owl:NamedIndividual>
    


    <!-- http://purl.obolibrary.org/obo/GAZ_00612972 -->

    <owl:NamedIndividual rdf:about="http://purl.obolibrary.org/obo/GAZ_00612972">
        <obo:IAO_0000115>A river.</obo:IAO_0000115>
        <oboInOwl:hasOBONamespace>GAZ</oboInOwl:hasOBONamespace>
        <oboInOwl:id>GAZ:00612972</oboInOwl:id>
        <rdfs:label>Riebgraben</rdfs:label>
    </owl:NamedIndividual>
    


    <!-- http://purl.obolibrary.org/obo/GAZ_00612973 -->

    <owl:NamedIndividual rdf:about="http://purl.obolibrary.org/obo/GAZ_00612973">
        <obo:IAO_0000115>A river.</obo:IAO_0000115>
        <oboInOwl:hasOBONamespace>GAZ</oboInOwl:hasOBONamespace>
        <oboInOwl:id>GAZ:00612973</oboInOwl:id>
        <rdfs:label>Trogellahnegraben</rdfs:label>
    </owl:NamedIndividual>
    


    <!-- http://purl.obolibrary.org/obo/GAZ_00612974 -->

    <owl:NamedIndividual rdf:about="http://purl.obolibrary.org/obo/GAZ_00612974">
        <obo:IAO_0000115>A river.</obo:IAO_0000115>
        <oboInOwl:hasOBONamespace>GAZ</oboInOwl:hasOBONamespace>
        <oboInOwl:id>GAZ:00612974</oboInOwl:id>
        <rdfs:label>Leimbach</rdfs:label>
    </owl:NamedIndividual>
    


    <!-- http://purl.obolibrary.org/obo/GAZ_00613056 -->

    <owl:NamedIndividual rdf:about="http://purl.obolibrary.org/obo/GAZ_00613056">
        <obo:IAO_0000115>A reservoir.</obo:IAO_0000115>
        <oboInOwl:hasOBONamespace>GAZ</oboInOwl:hasOBONamespace>
        <oboInOwl:id>GAZ:00613056</oboInOwl:id>
        <rdfs:label>Stausee Altheim</rdfs:label>
    </owl:NamedIndividual>
    


    <!-- http://purl.obolibrary.org/obo/GAZ_00613057 -->

    <owl:NamedIndividual rdf:about="http://purl.obolibrary.org/obo/GAZ_00613057">
        <obo:IAO_0000115>A reservoir.</obo:IAO_0000115>
        <oboInOwl:hasOBONamespace>GAZ</oboInOwl:hasOBONamespace>
        <oboInOwl:id>GAZ:00613057</oboInOwl:id>
        <rdfs:label>Stauweiher</rdfs:label>
    </owl:NamedIndividual>
    


    <!-- http://purl.obolibrary.org/obo/GAZ_00613058 -->

    <owl:NamedIndividual rdf:about="http://purl.obolibrary.org/obo/GAZ_00613058">
        <obo:IAO_0000115>A reservoir.</obo:IAO_0000115>
        <oboInOwl:hasOBONamespace>GAZ</oboInOwl:hasOBONamespace>
        <oboInOwl:id>GAZ:00613058</oboInOwl:id>
        <rdfs:label>Stausee Niederaichbach</rdfs:label>
    </owl:NamedIndividual>
    


    <!-- http://purl.obolibrary.org/obo/GAZ_00619830 -->

    <owl:NamedIndividual rdf:about="http://purl.obolibrary.org/obo/GAZ_00619830"/>
    


    <!-- http://purl.obolibrary.org/obo/GAZ_00619876 -->

    <owl:NamedIndividual rdf:about="http://purl.obolibrary.org/obo/GAZ_00619876">
        <obo:IAO_0000115>A hydroelectric power station.</obo:IAO_0000115>
        <oboInOwl:hasOBONamespace>GAZ</oboInOwl:hasOBONamespace>
        <oboInOwl:id>GAZ:00619876</oboInOwl:id>
        <rdfs:label>Isarwerk 1</rdfs:label>
    </owl:NamedIndividual>
    


    <!-- http://purl.obolibrary.org/obo/GAZ_00619897 -->

    <owl:NamedIndividual rdf:about="http://purl.obolibrary.org/obo/GAZ_00619897">
        <obo:RO_0001025 rdf:resource="http://purl.obolibrary.org/obo/GAZ_00619830"/>
        <obo:IAO_0000115>A hydroelectric power station.</obo:IAO_0000115>
        <oboInOwl:hasOBONamespace>GAZ</oboInOwl:hasOBONamespace>
        <oboInOwl:id>GAZ:00619897</oboInOwl:id>
        <rdfs:label>Isarwerk 2</rdfs:label>
    </owl:NamedIndividual>
    


    <!-- http://purl.obolibrary.org/obo/GAZ_00619898 -->

    <owl:NamedIndividual rdf:about="http://purl.obolibrary.org/obo/GAZ_00619898">
        <obo:RO_0001025 rdf:resource="http://purl.obolibrary.org/obo/GAZ_00619830"/>
        <oboInOwl:hasOBONamespace>GAZ</oboInOwl:hasOBONamespace>
        <oboInOwl:id>GAZ:00619898</oboInOwl:id>
        <rdfs:label>Isarwerk 3</rdfs:label>
    </owl:NamedIndividual>
    


    <!-- http://purl.obolibrary.org/obo/GAZ_00619923 -->

    <owl:NamedIndividual rdf:about="http://purl.obolibrary.org/obo/GAZ_00619923">
        <rdf:type rdf:resource="http://purl.obolibrary.org/obo/ENVO_00000423"/>
        <obo:IAO_0000115>A fluvial island.</obo:IAO_0000115>
        <oboInOwl:hasOBONamespace>GAZ</oboInOwl:hasOBONamespace>
        <oboInOwl:id>GAZ:00619923</oboInOwl:id>
        <rdfs:label>Feuerwerksinsel</rdfs:label>
    </owl:NamedIndividual>
    


    <!-- http://purl.obolibrary.org/obo/GAZ_00619924 -->

    <owl:NamedIndividual rdf:about="http://purl.obolibrary.org/obo/GAZ_00619924">
        <rdf:type rdf:resource="http://purl.obolibrary.org/obo/ENVO_00000423"/>
        <obo:IAO_0000115>A fluvial island.</obo:IAO_0000115>
        <oboInOwl:hasOBONamespace>GAZ</oboInOwl:hasOBONamespace>
        <oboInOwl:id>GAZ:00619924</oboInOwl:id>
        <rdfs:label>Kalkinsel</rdfs:label>
    </owl:NamedIndividual>
    


    <!-- http://purl.obolibrary.org/obo/GAZ_00621614 -->

    <owl:NamedIndividual rdf:about="http://purl.obolibrary.org/obo/GAZ_00621614">
        <obo:IAO_0000115>A canal.</obo:IAO_0000115>
        <oboInOwl:hasOBONamespace>GAZ</oboInOwl:hasOBONamespace>
        <oboInOwl:id>GAZ:00621614</oboInOwl:id>
        <rdfs:label>Muhlbach</rdfs:label>
    </owl:NamedIndividual>
    


    <!-- http://purl.obolibrary.org/obo/GAZ_00621615 -->

    <owl:NamedIndividual rdf:about="http://purl.obolibrary.org/obo/GAZ_00621615">
        <obo:IAO_0000115>A populated place. A region of Dachau.</obo:IAO_0000115>
        <oboInOwl:hasOBONamespace>GAZ</oboInOwl:hasOBONamespace>
        <oboInOwl:id>GAZ:00621615</oboInOwl:id>
        <rdfs:label>Schleissheimer Kanal</rdfs:label>
    </owl:NamedIndividual>
    


    <!-- http://purl.obolibrary.org/obo/GAZ_00622496 -->

    <owl:NamedIndividual rdf:about="http://purl.obolibrary.org/obo/GAZ_00622496">
        <obo:IAO_0000115>A hydroelectric power station.</obo:IAO_0000115>
        <oboInOwl:hasOBONamespace>GAZ</oboInOwl:hasOBONamespace>
        <oboInOwl:id>GAZ:00622496</oboInOwl:id>
        <rdfs:label>Kraftwerk Neufinsing</rdfs:label>
    </owl:NamedIndividual>
    


    <!-- http://purl.obolibrary.org/obo/GAZ_00622497 -->

    <owl:NamedIndividual rdf:about="http://purl.obolibrary.org/obo/GAZ_00622497">
        <obo:IAO_0000115>A hydroelectric power station.</obo:IAO_0000115>
        <oboInOwl:hasOBONamespace>GAZ</oboInOwl:hasOBONamespace>
        <oboInOwl:id>GAZ:00622497</oboInOwl:id>
        <rdfs:label>Speicherseekraftwerk Ismaning</rdfs:label>
    </owl:NamedIndividual>
    


    <!-- http://purl.obolibrary.org/obo/GAZ_00622498 -->

    <owl:NamedIndividual rdf:about="http://purl.obolibrary.org/obo/GAZ_00622498">
        <obo:IAO_0000115>A hydroelectric power station.</obo:IAO_0000115>
        <oboInOwl:hasOBONamespace>GAZ</oboInOwl:hasOBONamespace>
        <oboInOwl:id>GAZ:00622498</oboInOwl:id>
        <rdfs:label>Kraftwerk Aufkirchen</rdfs:label>
    </owl:NamedIndividual>
    


    <!-- http://purl.obolibrary.org/obo/GAZ_00622499 -->

    <owl:NamedIndividual rdf:about="http://purl.obolibrary.org/obo/GAZ_00622499">
        <obo:IAO_0000115>A hydroelectric power station.</obo:IAO_0000115>
        <oboInOwl:hasOBONamespace>GAZ</oboInOwl:hasOBONamespace>
        <oboInOwl:id>GAZ:00622499</oboInOwl:id>
        <rdfs:label>Kraftwerk Eitting</rdfs:label>
    </owl:NamedIndividual>
    


    <!-- http://purl.obolibrary.org/obo/GAZ_00622501 -->

    <owl:NamedIndividual rdf:about="http://purl.obolibrary.org/obo/GAZ_00622501">
        <obo:IAO_0000115>A river.</obo:IAO_0000115>
        <oboInOwl:hasOBONamespace>GAZ</oboInOwl:hasOBONamespace>
        <oboInOwl:id>GAZ:00622501</oboInOwl:id>
        <rdfs:label>Anzinger Sempt</rdfs:label>
    </owl:NamedIndividual>
    


    <!-- http://purl.obolibrary.org/obo/GAZ_00623318 -->

    <owl:NamedIndividual rdf:about="http://purl.obolibrary.org/obo/GAZ_00623318">
        <obo:IAO_0000115>A protected area.</obo:IAO_0000115>
        <oboInOwl:hasOBONamespace>GAZ</oboInOwl:hasOBONamespace>
        <oboInOwl:id>GAZ:00623318</oboInOwl:id>
        <rdfs:label>Vogelfreistatte Mittlere Isarstauseen</rdfs:label>
    </owl:NamedIndividual>
    


    <!-- http://purl.obolibrary.org/obo/GAZ_00623319 -->

    <owl:NamedIndividual rdf:about="http://purl.obolibrary.org/obo/GAZ_00623319">
        <obo:RO_0001025 rdf:resource="http://purl.obolibrary.org/obo/GAZ_00623318"/>
        <obo:IAO_0000115>Lakes.</obo:IAO_0000115>
        <oboInOwl:hasOBONamespace>GAZ</oboInOwl:hasOBONamespace>
        <oboInOwl:id>GAZ:00623319</oboInOwl:id>
        <rdfs:label>Isarstauseen</rdfs:label>
    </owl:NamedIndividual>
    


    <!-- http://purl.obolibrary.org/obo/GAZ_00623489 -->

    <owl:NamedIndividual rdf:about="http://purl.obolibrary.org/obo/GAZ_00623489">
        <obo:IAO_0000115>A hydroelectric power station.</obo:IAO_0000115>
        <oboInOwl:hasOBONamespace>GAZ</oboInOwl:hasOBONamespace>
        <oboInOwl:id>GAZ:00623489</oboInOwl:id>
        <rdfs:label>Wasserkraftwerk an der Ampe</rdfs:label>
    </owl:NamedIndividual>
    


    <!-- http://purl.obolibrary.org/obo/GAZ_00623580 -->

    <owl:NamedIndividual rdf:about="http://purl.obolibrary.org/obo/GAZ_00623580">
        <obo:IAO_0000115>A river.</obo:IAO_0000115>
        <oboInOwl:hasOBONamespace>GAZ</oboInOwl:hasOBONamespace>
        <oboInOwl:id>GAZ:00623580</oboInOwl:id>
        <rdfs:label>Stauwehr Krun</rdfs:label>
    </owl:NamedIndividual>
    


    <!-- http://purl.obolibrary.org/obo/GAZ_00626162 -->

    <owl:NamedIndividual rdf:about="http://purl.obolibrary.org/obo/GAZ_00626162">
        <obo:IAO_0000115>A populated place. A district (Ortsteil).</obo:IAO_0000115>
        <oboInOwl:hasOBONamespace>GAZ</oboInOwl:hasOBONamespace>
        <oboInOwl:id>GAZ:00626162</oboInOwl:id>
        <rdfs:label>Leitzachwerke</rdfs:label>
    </owl:NamedIndividual>
    


    <!-- http://purl.obolibrary.org/obo/GAZ_00630339 -->

    <owl:NamedIndividual rdf:about="http://purl.obolibrary.org/obo/GAZ_00630339">
        <obo:IAO_0000115>A river.</obo:IAO_0000115>
        <oboInOwl:hasOBONamespace>GAZ</oboInOwl:hasOBONamespace>
        <oboInOwl:id>GAZ:00630339</oboInOwl:id>
        <rdfs:label>Kohlersgrundbach</rdfs:label>
    </owl:NamedIndividual>
    


    <!-- http://purl.obolibrary.org/obo/GAZ_00633599 -->

    <owl:NamedIndividual rdf:about="http://purl.obolibrary.org/obo/GAZ_00633599">
        <obo:IAO_0000115>A river.</obo:IAO_0000115>
        <oboInOwl:hasOBONamespace>GAZ</oboInOwl:hasOBONamespace>
        <oboInOwl:id>GAZ:00633599</oboInOwl:id>
        <rdfs:label>Hochgraben</rdfs:label>
    </owl:NamedIndividual>
    


    <!-- http://purl.obolibrary.org/obo/GAZ_00633600 -->

    <owl:NamedIndividual rdf:about="http://purl.obolibrary.org/obo/GAZ_00633600">
        <obo:IAO_0000115>A river.</obo:IAO_0000115>
        <oboInOwl:hasOBONamespace>GAZ</oboInOwl:hasOBONamespace>
        <oboInOwl:id>GAZ:00633600</oboInOwl:id>
        <rdfs:label>Vogtendorfer Grundbach</rdfs:label>
    </owl:NamedIndividual>
    


    <!-- http://purl.obolibrary.org/obo/GAZ_00635572 -->

    <owl:NamedIndividual rdf:about="http://purl.obolibrary.org/obo/GAZ_00635572">
        <obo:IAO_0000115>A lock.</obo:IAO_0000115>
        <oboInOwl:hasOBONamespace>GAZ</oboInOwl:hasOBONamespace>
        <oboInOwl:id>GAZ:00635572</oboInOwl:id>
        <rdfs:label>Schleuse Bamberg</rdfs:label>
    </owl:NamedIndividual>
    


    <!-- http://purl.obolibrary.org/obo/GAZ_00635573 -->

    <owl:NamedIndividual rdf:about="http://purl.obolibrary.org/obo/GAZ_00635573">
        <obo:IAO_0000115>A lock.</obo:IAO_0000115>
        <oboInOwl:hasOBONamespace>GAZ</oboInOwl:hasOBONamespace>
        <oboInOwl:id>GAZ:00635573</oboInOwl:id>
        <rdfs:label>Schleuse Strullendorf</rdfs:label>
    </owl:NamedIndividual>
    


    <!-- http://purl.obolibrary.org/obo/GAZ_00635574 -->

    <owl:NamedIndividual rdf:about="http://purl.obolibrary.org/obo/GAZ_00635574">
        <obo:IAO_0000115>A lock.</obo:IAO_0000115>
        <oboInOwl:hasOBONamespace>GAZ</oboInOwl:hasOBONamespace>
        <oboInOwl:id>GAZ:00635574</oboInOwl:id>
        <rdfs:label>Schleuse Forchheim</rdfs:label>
    </owl:NamedIndividual>
    


    <!-- http://purl.obolibrary.org/obo/GAZ_00635575 -->

    <owl:NamedIndividual rdf:about="http://purl.obolibrary.org/obo/GAZ_00635575">
        <obo:IAO_0000115>A lock.</obo:IAO_0000115>
        <oboInOwl:hasOBONamespace>GAZ</oboInOwl:hasOBONamespace>
        <oboInOwl:id>GAZ:00635575</oboInOwl:id>
        <rdfs:label>Schleuse Hausen</rdfs:label>
    </owl:NamedIndividual>
    


    <!-- http://purl.obolibrary.org/obo/GAZ_00635576 -->

    <owl:NamedIndividual rdf:about="http://purl.obolibrary.org/obo/GAZ_00635576">
        <obo:IAO_0000115>A lock.</obo:IAO_0000115>
        <oboInOwl:hasOBONamespace>GAZ</oboInOwl:hasOBONamespace>
        <oboInOwl:id>GAZ:00635576</oboInOwl:id>
        <rdfs:label>Schleuse Erlangen</rdfs:label>
    </owl:NamedIndividual>
    


    <!-- http://purl.obolibrary.org/obo/GAZ_00635577 -->

    <owl:NamedIndividual rdf:about="http://purl.obolibrary.org/obo/GAZ_00635577">
        <obo:IAO_0000115>A lock.</obo:IAO_0000115>
        <oboInOwl:hasOBONamespace>GAZ</oboInOwl:hasOBONamespace>
        <oboInOwl:id>GAZ:00635577</oboInOwl:id>
        <rdfs:label>Schleuse Kriegenbrunn</rdfs:label>
    </owl:NamedIndividual>
    


    <!-- http://purl.obolibrary.org/obo/GAZ_00635578 -->

    <owl:NamedIndividual rdf:about="http://purl.obolibrary.org/obo/GAZ_00635578">
        <obo:IAO_0000115>A lock.</obo:IAO_0000115>
        <oboInOwl:hasOBONamespace>GAZ</oboInOwl:hasOBONamespace>
        <oboInOwl:id>GAZ:00635578</oboInOwl:id>
        <rdfs:label>Schleuse Nurnberg</rdfs:label>
    </owl:NamedIndividual>
    


    <!-- http://purl.obolibrary.org/obo/GAZ_00635579 -->

    <owl:NamedIndividual rdf:about="http://purl.obolibrary.org/obo/GAZ_00635579">
        <obo:IAO_0000115>A lock.</obo:IAO_0000115>
        <oboInOwl:hasOBONamespace>GAZ</oboInOwl:hasOBONamespace>
        <oboInOwl:id>GAZ:00635579</oboInOwl:id>
        <rdfs:label>Schleuse Eibach</rdfs:label>
    </owl:NamedIndividual>
    


    <!-- http://purl.obolibrary.org/obo/GAZ_00635580 -->

    <owl:NamedIndividual rdf:about="http://purl.obolibrary.org/obo/GAZ_00635580">
        <obo:IAO_0000115>A lock.</obo:IAO_0000115>
        <oboInOwl:hasOBONamespace>GAZ</oboInOwl:hasOBONamespace>
        <oboInOwl:id>GAZ:00635580</oboInOwl:id>
        <rdfs:label>Schleuse Eckersmuhlen</rdfs:label>
    </owl:NamedIndividual>
    


    <!-- http://purl.obolibrary.org/obo/GAZ_00635581 -->

    <owl:NamedIndividual rdf:about="http://purl.obolibrary.org/obo/GAZ_00635581">
        <obo:IAO_0000115>A lock.</obo:IAO_0000115>
        <oboInOwl:hasOBONamespace>GAZ</oboInOwl:hasOBONamespace>
        <oboInOwl:id>GAZ:00635581</oboInOwl:id>
        <rdfs:label>Schleuse Hilpoltstein</rdfs:label>
    </owl:NamedIndividual>
    


    <!-- http://purl.obolibrary.org/obo/GAZ_00635582 -->

    <owl:NamedIndividual rdf:about="http://purl.obolibrary.org/obo/GAZ_00635582">
        <obo:IAO_0000115>A lock.</obo:IAO_0000115>
        <oboInOwl:hasOBONamespace>GAZ</oboInOwl:hasOBONamespace>
        <oboInOwl:id>GAZ:00635582</oboInOwl:id>
        <rdfs:label>Schleuse Bachhausen</rdfs:label>
    </owl:NamedIndividual>
    


    <!-- http://purl.obolibrary.org/obo/GAZ_00635583 -->

    <owl:NamedIndividual rdf:about="http://purl.obolibrary.org/obo/GAZ_00635583">
        <obo:IAO_0000115>A populated place. A City district (Stadtteil).</obo:IAO_0000115>
        <oboInOwl:hasOBONamespace>GAZ</oboInOwl:hasOBONamespace>
        <oboInOwl:id>GAZ:00635583</oboInOwl:id>
        <rdfs:label>Schleuse Berching</rdfs:label>
    </owl:NamedIndividual>
    


    <!-- http://purl.obolibrary.org/obo/GAZ_00635584 -->

    <owl:NamedIndividual rdf:about="http://purl.obolibrary.org/obo/GAZ_00635584">
        <obo:IAO_0000115>A populated place. A City district (Stadtteil).</obo:IAO_0000115>
        <oboInOwl:hasOBONamespace>GAZ</oboInOwl:hasOBONamespace>
        <oboInOwl:id>GAZ:00635584</oboInOwl:id>
        <rdfs:label>Schleuse Dietfurt</rdfs:label>
    </owl:NamedIndividual>
    


    <!-- http://purl.obolibrary.org/obo/GAZ_00635585 -->

    <owl:NamedIndividual rdf:about="http://purl.obolibrary.org/obo/GAZ_00635585">
        <obo:IAO_0000115>A lock.</obo:IAO_0000115>
        <oboInOwl:hasOBONamespace>GAZ</oboInOwl:hasOBONamespace>
        <oboInOwl:id>GAZ:00635585</oboInOwl:id>
        <rdfs:label>Schleuse Riedenburg</rdfs:label>
    </owl:NamedIndividual>
    


    <!-- http://purl.obolibrary.org/obo/GAZ_00635586 -->

    <owl:NamedIndividual rdf:about="http://purl.obolibrary.org/obo/GAZ_00635586">
        <obo:IAO_0000115>A lock.</obo:IAO_0000115>
        <oboInOwl:hasOBONamespace>GAZ</oboInOwl:hasOBONamespace>
        <oboInOwl:id>GAZ:00635586</oboInOwl:id>
        <rdfs:label>Schleuse Kelheim</rdfs:label>
    </owl:NamedIndividual>
    


    <!-- http://purl.obolibrary.org/obo/GAZ_00639825 -->

    <owl:NamedIndividual rdf:about="http://purl.obolibrary.org/obo/GAZ_00639825">
        <obo:RO_0001025 rdf:resource="http://purl.obolibrary.org/obo/GAZ_00056796"/>
        <obo:IAO_0000115>A glacier.</obo:IAO_0000115>
        <oboInOwl:hasOBONamespace>GAZ</oboInOwl:hasOBONamespace>
        <oboInOwl:id>GAZ:00639825</oboInOwl:id>
        <rdfs:label>Blaueis</rdfs:label>
    </owl:NamedIndividual>
    


    <!-- http://purl.obolibrary.org/obo/GAZ_00641183 -->

    <owl:NamedIndividual rdf:about="http://purl.obolibrary.org/obo/GAZ_00641183">
        <obo:RO_0001025 rdf:resource="http://purl.obolibrary.org/obo/GAZ_00261031"/>
        <obo:IAO_0000115>A glacier.</obo:IAO_0000115>
        <oboInOwl:hasOBONamespace>GAZ</oboInOwl:hasOBONamespace>
        <oboInOwl:id>GAZ:00641183</oboInOwl:id>
        <rdfs:label>Obersulzbachkees</rdfs:label>
    </owl:NamedIndividual>
    


    <!-- http://purl.obolibrary.org/obo/GAZ_00641263 -->

    <owl:NamedIndividual rdf:about="http://purl.obolibrary.org/obo/GAZ_00641263">
        <obo:RO_0001025 rdf:resource="http://purl.obolibrary.org/obo/GAZ_00056796"/>
        <obo:IAO_0000115>A glacier (now much reduced in extent).</obo:IAO_0000115>
        <oboInOwl:hasOBONamespace>GAZ</oboInOwl:hasOBONamespace>
        <oboInOwl:id>GAZ:00641263</oboInOwl:id>
        <rdfs:label>Ubergossene Alm</rdfs:label>
    </owl:NamedIndividual>
    


    <!-- http://purl.obolibrary.org/obo/GAZ_00644972 -->

    <owl:NamedIndividual rdf:about="http://purl.obolibrary.org/obo/GAZ_00644972">
        <obo:RO_0001025 rdf:resource="http://purl.obolibrary.org/obo/GAZ_00008111"/>
        <obo:IAO_0000115>A lacustrine land-tied island.</obo:IAO_0000115>
        <oboInOwl:hasOBONamespace>GAZ</oboInOwl:hasOBONamespace>
        <oboInOwl:id>GAZ:00644972</oboInOwl:id>
        <rdfs:label>Insel Lindau</rdfs:label>
    </owl:NamedIndividual>
    


    <!-- http://purl.obolibrary.org/obo/GAZ_00645377 -->

    <owl:NamedIndividual rdf:about="http://purl.obolibrary.org/obo/GAZ_00645377">
        <obo:IAO_0000115>A lake.</obo:IAO_0000115>
        <oboInOwl:hasOBONamespace>GAZ</oboInOwl:hasOBONamespace>
        <oboInOwl:id>GAZ:00645377</oboInOwl:id>
        <rdfs:label>Leckner See</rdfs:label>
    </owl:NamedIndividual>
    


    <!-- http://purl.obolibrary.org/obo/GAZ_00646552 -->

    <owl:NamedIndividual rdf:about="http://purl.obolibrary.org/obo/GAZ_00646552">
        <obo:IAO_0000115>A harbor.</obo:IAO_0000115>
        <oboInOwl:hasOBONamespace>GAZ</oboInOwl:hasOBONamespace>
        <oboInOwl:id>GAZ:00646552</oboInOwl:id>
        <rdfs:label>Bayernhafen Aschaffenburg</rdfs:label>
    </owl:NamedIndividual>
    


    <!-- http://purl.obolibrary.org/obo/GAZ_00646553 -->

    <owl:NamedIndividual rdf:about="http://purl.obolibrary.org/obo/GAZ_00646553">
        <obo:IAO_0000115>A harbor.</obo:IAO_0000115>
        <oboInOwl:hasOBONamespace>GAZ</oboInOwl:hasOBONamespace>
        <oboInOwl:id>GAZ:00646553</oboInOwl:id>
        <rdfs:label>Bayernhafen Bamberg</rdfs:label>
    </owl:NamedIndividual>
    


    <!-- http://purl.obolibrary.org/obo/GAZ_00646554 -->

    <owl:NamedIndividual rdf:about="http://purl.obolibrary.org/obo/GAZ_00646554">
        <obo:IAO_0000115>A harbor.</obo:IAO_0000115>
        <oboInOwl:hasOBONamespace>GAZ</oboInOwl:hasOBONamespace>
        <oboInOwl:id>GAZ:00646554</oboInOwl:id>
        <rdfs:label>Bayernhafen Nurnberg</rdfs:label>
    </owl:NamedIndividual>
    


    <!-- http://purl.obolibrary.org/obo/GAZ_00646555 -->

    <owl:NamedIndividual rdf:about="http://purl.obolibrary.org/obo/GAZ_00646555">
        <obo:IAO_0000115>A harbor.</obo:IAO_0000115>
        <oboInOwl:hasOBONamespace>GAZ</oboInOwl:hasOBONamespace>
        <oboInOwl:id>GAZ:00646555</oboInOwl:id>
        <rdfs:label>Bayernhafen Roth</rdfs:label>
    </owl:NamedIndividual>
    


    <!-- http://purl.obolibrary.org/obo/GAZ_00647476 -->

    <owl:NamedIndividual rdf:about="http://purl.obolibrary.org/obo/GAZ_00647476">
        <obo:IAO_0000115>A fluvial island; between the main arm of the Main and the Mainkanal between Volkach and Gerlachshausen.</obo:IAO_0000115>
        <oboInOwl:hasOBONamespace>GAZ</oboInOwl:hasOBONamespace>
        <oboInOwl:id>GAZ:00647476</oboInOwl:id>
        <rdfs:label>Weininsel</rdfs:label>
    </owl:NamedIndividual>
    


    <!-- http://purl.obolibrary.org/obo/GAZ_00647961 -->

    <owl:NamedIndividual rdf:about="http://purl.obolibrary.org/obo/GAZ_00647961">
        <obo:IAO_0000115>A lock.</obo:IAO_0000115>
        <oboInOwl:hasOBONamespace>GAZ</oboInOwl:hasOBONamespace>
        <oboInOwl:id>GAZ:00647961</oboInOwl:id>
        <rdfs:label>Schleuse Faulbach</rdfs:label>
    </owl:NamedIndividual>
    


    <!-- http://purl.obolibrary.org/obo/GAZ_00648828 -->

    <owl:NamedIndividual rdf:about="http://purl.obolibrary.org/obo/GAZ_00648828">
        <obo:RO_0001025 rdf:resource="http://purl.obolibrary.org/obo/GAZ_00060656"/>
        <obo:IAO_0000115>A mountain; the highest in Germany.</obo:IAO_0000115>
        <oboInOwl:hasOBONamespace>GAZ</oboInOwl:hasOBONamespace>
        <oboInOwl:id>GAZ:00648828</oboInOwl:id>
        <rdfs:label>Zugspitze</rdfs:label>
    </owl:NamedIndividual>
    


    <!-- http://purl.obolibrary.org/obo/GAZ_00648829 -->

    <owl:NamedIndividual rdf:about="http://purl.obolibrary.org/obo/GAZ_00648829">
        <obo:RO_0001025 rdf:resource="http://purl.obolibrary.org/obo/GAZ_00648828"/>
        <obo:IAO_0000115>A glacier.</obo:IAO_0000115>
        <oboInOwl:hasOBONamespace>GAZ</oboInOwl:hasOBONamespace>
        <oboInOwl:id>GAZ:00648829</oboInOwl:id>
        <rdfs:label>Nordliche Schneeferner</rdfs:label>
    </owl:NamedIndividual>
    


    <!-- http://purl.obolibrary.org/obo/GAZ_00648830 -->

    <owl:NamedIndividual rdf:about="http://purl.obolibrary.org/obo/GAZ_00648830">
        <obo:RO_0001025 rdf:resource="http://purl.obolibrary.org/obo/GAZ_00648828"/>
        <obo:IAO_0000115>A glacier.</obo:IAO_0000115>
        <oboInOwl:hasOBONamespace>GAZ</oboInOwl:hasOBONamespace>
        <oboInOwl:id>GAZ:00648830</oboInOwl:id>
        <rdfs:label>Hollentalferner</rdfs:label>
    </owl:NamedIndividual>
    


    <!-- http://purl.obolibrary.org/obo/GAZ_00648831 -->

    <owl:NamedIndividual rdf:about="http://purl.obolibrary.org/obo/GAZ_00648831">
        <obo:RO_0001025 rdf:resource="http://purl.obolibrary.org/obo/GAZ_00648828"/>
        <obo:IAO_0000115>A glacier.</obo:IAO_0000115>
        <oboInOwl:hasOBONamespace>GAZ</oboInOwl:hasOBONamespace>
        <oboInOwl:id>GAZ:00648831</oboInOwl:id>
        <rdfs:label>Sudliche Schneeferner</rdfs:label>
    </owl:NamedIndividual>
    


    <!-- http://purl.obolibrary.org/obo/GAZ_00648834 -->

    <owl:NamedIndividual rdf:about="http://purl.obolibrary.org/obo/GAZ_00648834">
        <obo:RO_0001025 rdf:resource="http://purl.obolibrary.org/obo/GAZ_00060656"/>
        <obo:IAO_0000115>A protected area.</obo:IAO_0000115>
        <oboInOwl:hasOBONamespace>GAZ</oboInOwl:hasOBONamespace>
        <oboInOwl:id>GAZ:00648834</oboInOwl:id>
        <rdfs:label>Naturwaldreservat Wettersteinwald</rdfs:label>
    </owl:NamedIndividual>
    


    <!-- http://purl.obolibrary.org/obo/GAZ_00648981 -->

    <owl:NamedIndividual rdf:about="http://purl.obolibrary.org/obo/GAZ_00648981">
        <obo:IAO_0000115>A river.</obo:IAO_0000115>
        <oboInOwl:hasOBONamespace>GAZ</oboInOwl:hasOBONamespace>
        <oboInOwl:id>GAZ:00648981</oboInOwl:id>
        <rdfs:label>Krebsbach</rdfs:label>
    </owl:NamedIndividual>
    


    <!-- http://purl.obolibrary.org/obo/GAZ_00648985 -->

    <owl:NamedIndividual rdf:about="http://purl.obolibrary.org/obo/GAZ_00648985">
        <rdf:type rdf:resource="http://purl.obolibrary.org/obo/ENVO_00000080"/>
        <obo:RO_0001025 rdf:resource="http://purl.obolibrary.org/obo/GAZ_00056803"/>
        <obo:IAO_0000115>A mountain chain.</obo:IAO_0000115>
        <oboInOwl:hasOBONamespace>GAZ</oboInOwl:hasOBONamespace>
        <oboInOwl:id>GAZ:00648985</oboInOwl:id>
        <rdfs:label>Soierngruppe</rdfs:label>
    </owl:NamedIndividual>
    


    <!-- http://purl.obolibrary.org/obo/GAZ_00648986 -->

    <owl:NamedIndividual rdf:about="http://purl.obolibrary.org/obo/GAZ_00648986">
        <obo:RO_0001025 rdf:resource="http://purl.obolibrary.org/obo/GAZ_00648985"/>
        <obo:IAO_0000115>Lakes.</obo:IAO_0000115>
        <oboInOwl:hasOBONamespace>GAZ</oboInOwl:hasOBONamespace>
        <oboInOwl:id>GAZ:00648986</oboInOwl:id>
        <rdfs:label>Soiernseen</rdfs:label>
    </owl:NamedIndividual>
    


    <!-- http://purl.obolibrary.org/obo/GAZ_00650219 -->

    <owl:NamedIndividual rdf:about="http://purl.obolibrary.org/obo/GAZ_00650219">
        <obo:IAO_0000115>A populated place. A district (Ortsteil).</obo:IAO_0000115>
        <oboInOwl:hasOBONamespace>GAZ</oboInOwl:hasOBONamespace>
        <oboInOwl:id>GAZ:00650219</oboInOwl:id>
        <rdfs:label>Kanalschleuse 28</rdfs:label>
    </owl:NamedIndividual>
    


    <!-- http://purl.obolibrary.org/obo/GAZ_00650220 -->

    <owl:NamedIndividual rdf:about="http://purl.obolibrary.org/obo/GAZ_00650220">
        <obo:IAO_0000115>A populated place. A district (Ortsteil).</obo:IAO_0000115>
        <oboInOwl:hasOBONamespace>GAZ</oboInOwl:hasOBONamespace>
        <oboInOwl:id>GAZ:00650220</oboInOwl:id>
        <rdfs:label>Kanalschleuse 29</rdfs:label>
    </owl:NamedIndividual>
    


    <!-- http://purl.obolibrary.org/obo/GAZ_00650221 -->

    <owl:NamedIndividual rdf:about="http://purl.obolibrary.org/obo/GAZ_00650221">
        <obo:IAO_0000115>A populated place. A district (Ortsteil).</obo:IAO_0000115>
        <oboInOwl:hasOBONamespace>GAZ</oboInOwl:hasOBONamespace>
        <oboInOwl:id>GAZ:00650221</oboInOwl:id>
        <rdfs:label>Kanalschleuse 30</rdfs:label>
    </owl:NamedIndividual>
    


    <!-- http://purl.obolibrary.org/obo/GAZ_00650466 -->

    <owl:NamedIndividual rdf:about="http://purl.obolibrary.org/obo/GAZ_00650466">
        <obo:RO_0001025 rdf:resource="http://purl.obolibrary.org/obo/GAZ_00650467"/>
        <obo:IAO_0000115>A cave system; show caves.</obo:IAO_0000115>
        <oboInOwl:hasOBONamespace>GAZ</oboInOwl:hasOBONamespace>
        <oboInOwl:id>GAZ:00650466</oboInOwl:id>
        <rdfs:label>Salzgrabenhohle</rdfs:label>
    </owl:NamedIndividual>
    


    <!-- http://purl.obolibrary.org/obo/GAZ_00650467 -->

    <owl:NamedIndividual rdf:about="http://purl.obolibrary.org/obo/GAZ_00650467">
        <obo:RO_0001025 rdf:resource="http://purl.obolibrary.org/obo/GAZ_00056796"/>
        <obo:IAO_0000115>A high karst plateau in the Northern Limestone Alps. As one of the nine sub-ranges of the Berchtesgaden Alps the Steinernes Meer belongs partly to Bavaria and partly to Salzburg.</obo:IAO_0000115>
        <oboInOwl:hasOBONamespace>GAZ</oboInOwl:hasOBONamespace>
        <oboInOwl:id>GAZ:00650467</oboInOwl:id>
        <rdfs:label>Steinernes Meer</rdfs:label>
    </owl:NamedIndividual>
    


    <!-- http://purl.obolibrary.org/obo/GAZ_00650468 -->

    <owl:NamedIndividual rdf:about="http://purl.obolibrary.org/obo/GAZ_00650468">
        <obo:RO_0001025 rdf:resource="http://purl.obolibrary.org/obo/GAZ_00056796"/>
        <obo:IAO_0000115>An ice cave.</obo:IAO_0000115>
        <oboInOwl:hasOBONamespace>GAZ</oboInOwl:hasOBONamespace>
        <oboInOwl:id>GAZ:00650468</oboInOwl:id>
        <rdfs:label>Schellenberger Eishohle</rdfs:label>
    </owl:NamedIndividual>
    


    <!-- http://purl.obolibrary.org/obo/GAZ_00650472 -->

    <owl:NamedIndividual rdf:about="http://purl.obolibrary.org/obo/GAZ_00650472">
        <obo:RO_0001025 rdf:resource="http://purl.obolibrary.org/obo/GAZ_00060652"/>
        <obo:IAO_0000115>A mountain range. The easternmost part of the Bavarian Prealps.</obo:IAO_0000115>
        <oboInOwl:hasOBONamespace>GAZ</oboInOwl:hasOBONamespace>
        <oboInOwl:id>GAZ:00650472</oboInOwl:id>
        <rdfs:label>Mangfallgebirge</rdfs:label>
    </owl:NamedIndividual>
    


    <!-- http://purl.obolibrary.org/obo/GAZ_00650473 -->

    <owl:NamedIndividual rdf:about="http://purl.obolibrary.org/obo/GAZ_00650473">
        <obo:RO_0001025 rdf:resource="http://purl.obolibrary.org/obo/GAZ_00650472"/>
        <obo:IAO_0000115>A mountain massif.</obo:IAO_0000115>
        <oboInOwl:hasOBONamespace>GAZ</oboInOwl:hasOBONamespace>
        <oboInOwl:id>GAZ:00650473</oboInOwl:id>
        <rdfs:label>Wendelstein Massif</rdfs:label>
    </owl:NamedIndividual>
    


    <!-- http://purl.obolibrary.org/obo/GAZ_00650474 -->

    <owl:NamedIndividual rdf:about="http://purl.obolibrary.org/obo/GAZ_00650474">
        <obo:RO_0001025 rdf:resource="http://purl.obolibrary.org/obo/GAZ_00650473"/>
        <obo:IAO_0000115>A mountain. It lies between the valleys of the Leitzach and Inn.</obo:IAO_0000115>
        <oboInOwl:hasOBONamespace>GAZ</oboInOwl:hasOBONamespace>
        <oboInOwl:id>GAZ:00650474</oboInOwl:id>
        <rdfs:label>Wendelstein</rdfs:label>
    </owl:NamedIndividual>
    


    <!-- http://purl.obolibrary.org/obo/GAZ_00650475 -->

    <owl:NamedIndividual rdf:about="http://purl.obolibrary.org/obo/GAZ_00650475">
        <obo:RO_0001025 rdf:resource="http://purl.obolibrary.org/obo/GAZ_00650473"/>
        <obo:IAO_0000115>A cave.</obo:IAO_0000115>
        <oboInOwl:hasOBONamespace>GAZ</oboInOwl:hasOBONamespace>
        <oboInOwl:id>GAZ:00650475</oboInOwl:id>
        <rdfs:label>Wendelsteinhohle</rdfs:label>
    </owl:NamedIndividual>
    


    <!-- http://purl.obolibrary.org/obo/GAZ_00650500 -->

    <owl:NamedIndividual rdf:about="http://purl.obolibrary.org/obo/GAZ_00650500">
        <obo:RO_0001025 rdf:resource="http://purl.obolibrary.org/obo/GAZ_00056796"/>
        <obo:IAO_0000115>A mountain.</obo:IAO_0000115>
        <oboInOwl:hasOBONamespace>GAZ</oboInOwl:hasOBONamespace>
        <oboInOwl:id>GAZ:00650500</oboInOwl:id>
        <rdfs:label>Lattengebirge</rdfs:label>
    </owl:NamedIndividual>
    


    <!-- http://purl.obolibrary.org/obo/GAZ_00650501 -->

    <owl:NamedIndividual rdf:about="http://purl.obolibrary.org/obo/GAZ_00650501">
        <obo:RO_0001025 rdf:resource="http://purl.obolibrary.org/obo/GAZ_00650500"/>
        <obo:IAO_0000115>A lake.</obo:IAO_0000115>
        <oboInOwl:hasOBONamespace>GAZ</oboInOwl:hasOBONamespace>
        <oboInOwl:id>GAZ:00650501</oboInOwl:id>
        <rdfs:label>Steinbergsee</rdfs:label>
    </owl:NamedIndividual>
    


    <!-- http://purl.obolibrary.org/obo/GAZ_00650670 -->

    <owl:NamedIndividual rdf:about="http://purl.obolibrary.org/obo/GAZ_00650670">
        <obo:IAO_0000115>A river.</obo:IAO_0000115>
        <oboInOwl:hasOBONamespace>GAZ</oboInOwl:hasOBONamespace>
        <oboInOwl:id>GAZ:00650670</oboInOwl:id>
        <rdfs:label>Angerbach</rdfs:label>
    </owl:NamedIndividual>
    


    <!-- http://purl.obolibrary.org/obo/GAZ_00650671 -->

    <owl:NamedIndividual rdf:about="http://purl.obolibrary.org/obo/GAZ_00650671">
        <obo:IAO_0000115>A river.</obo:IAO_0000115>
        <oboInOwl:hasOBONamespace>GAZ</oboInOwl:hasOBONamespace>
        <oboInOwl:id>GAZ:00650671</oboInOwl:id>
        <rdfs:label>Grosskristenbach</rdfs:label>
    </owl:NamedIndividual>
    


    <!-- http://purl.obolibrary.org/obo/GAZ_00650673 -->

    <owl:NamedIndividual rdf:about="http://purl.obolibrary.org/obo/GAZ_00650673">
        <obo:IAO_0000115>A river.</obo:IAO_0000115>
        <oboInOwl:hasOBONamespace>GAZ</oboInOwl:hasOBONamespace>
        <oboInOwl:id>GAZ:00650673</oboInOwl:id>
        <rdfs:label>Reschenbach</rdfs:label>
    </owl:NamedIndividual>
    


    <!-- http://purl.obolibrary.org/obo/GAZ_00650698 -->

    <owl:NamedIndividual rdf:about="http://purl.obolibrary.org/obo/GAZ_00650698">
        <obo:IAO_0000115>A karst spring.</obo:IAO_0000115>
        <oboInOwl:hasOBONamespace>GAZ</oboInOwl:hasOBONamespace>
        <oboInOwl:id>GAZ:00650698</oboInOwl:id>
        <rdfs:label>Pegnitzquelle</rdfs:label>
    </owl:NamedIndividual>
    


    <!-- http://purl.obolibrary.org/obo/GAZ_00650735 -->

    <owl:NamedIndividual rdf:about="http://purl.obolibrary.org/obo/GAZ_00650735">
        <obo:IAO_0000115>A river.</obo:IAO_0000115>
        <oboInOwl:hasOBONamespace>GAZ</oboInOwl:hasOBONamespace>
        <oboInOwl:id>GAZ:00650735</oboInOwl:id>
        <rdfs:label>Weissbach [Lattengebirge]</rdfs:label>
    </owl:NamedIndividual>
    


    <!-- http://purl.obolibrary.org/obo/GAZ_00650736 -->

    <owl:NamedIndividual rdf:about="http://purl.obolibrary.org/obo/GAZ_00650736">
        <obo:RO_0001025 rdf:resource="http://purl.obolibrary.org/obo/GAZ_00650737"/>
        <obo:IAO_0000115>A mountain.</obo:IAO_0000115>
        <oboInOwl:hasOBONamespace>GAZ</oboInOwl:hasOBONamespace>
        <oboInOwl:id>GAZ:00650736</oboInOwl:id>
        <rdfs:label>Hoher Goll</rdfs:label>
    </owl:NamedIndividual>
    


    <!-- http://purl.obolibrary.org/obo/GAZ_00650737 -->

    <owl:NamedIndividual rdf:about="http://purl.obolibrary.org/obo/GAZ_00650737">
        <obo:RO_0001025 rdf:resource="http://purl.obolibrary.org/obo/GAZ_00056796"/>
        <obo:IAO_0000115>A mountain massiif. Rising above Obersalzberg near Berchtesgaden, the massif is situated between Lake Konigssee and the Konigsseer Ache in the west, opposite the Watzmann, and the Salzach Valley of the Tennengau region in the east. Neighbouring peaks include Hohes Brett, Jenner and the Kehlstein spur with the famous Kehlsteinhaus, linked with the Hoher Goll via the Mannlgrat ridge.</obo:IAO_0000115>
        <oboInOwl:hasOBONamespace>GAZ</oboInOwl:hasOBONamespace>
        <oboInOwl:id>GAZ:00650737</oboInOwl:id>
        <rdfs:label>Gollmassiv</rdfs:label>
    </owl:NamedIndividual>
    


    <!-- http://purl.obolibrary.org/obo/GAZ_00650738 -->

    <owl:NamedIndividual rdf:about="http://purl.obolibrary.org/obo/GAZ_00650738">
        <obo:RO_0001025 rdf:resource="http://purl.obolibrary.org/obo/GAZ_00650736"/>
        <obo:IAO_0000115>A cave.</obo:IAO_0000115>
        <oboInOwl:hasOBONamespace>GAZ</oboInOwl:hasOBONamespace>
        <oboInOwl:id>GAZ:00650738</oboInOwl:id>
        <rdfs:label>Schwarzbachfall-Hohle</rdfs:label>
    </owl:NamedIndividual>
    


    <!-- http://purl.obolibrary.org/obo/GAZ_00650746 -->

    <owl:NamedIndividual rdf:about="http://purl.obolibrary.org/obo/GAZ_00650746">
        <obo:RO_0001025 rdf:resource="http://purl.obolibrary.org/obo/GAZ_00051915"/>
        <obo:IAO_0000115>A mountain range, It is to the east of the Berchtesgaden Alps and the city of Salzburg.</obo:IAO_0000115>
        <oboInOwl:hasOBONamespace>GAZ</oboInOwl:hasOBONamespace>
        <oboInOwl:id>GAZ:00650746</oboInOwl:id>
        <rdfs:label>Salzkammergut-Berge</rdfs:label>
    </owl:NamedIndividual>
    


    <!-- http://purl.obolibrary.org/obo/GAZ_00650747 -->

    <owl:NamedIndividual rdf:about="http://purl.obolibrary.org/obo/GAZ_00650747">
        <obo:RO_0001025 rdf:resource="http://purl.obolibrary.org/obo/GAZ_00650746"/>
        <obo:IAO_0000115>A lake.</obo:IAO_0000115>
        <oboInOwl:hasOBONamespace>GAZ</oboInOwl:hasOBONamespace>
        <oboInOwl:id>GAZ:00650747</oboInOwl:id>
        <rdfs:label>Hintersee</rdfs:label>
    </owl:NamedIndividual>
    


    <!-- http://purl.obolibrary.org/obo/GAZ_00650748 -->

    <owl:NamedIndividual rdf:about="http://purl.obolibrary.org/obo/GAZ_00650748">
        <obo:RO_0001025 rdf:resource="http://purl.obolibrary.org/obo/GAZ_00103582"/>
        <obo:IAO_0000115>A lake.</obo:IAO_0000115>
        <oboInOwl:hasOBONamespace>GAZ</oboInOwl:hasOBONamespace>
        <oboInOwl:id>GAZ:00650748</oboInOwl:id>
        <rdfs:label>Jagersee</rdfs:label>
    </owl:NamedIndividual>
    


    <!-- http://purl.obolibrary.org/obo/GAZ_00650751 -->

    <owl:NamedIndividual rdf:about="http://purl.obolibrary.org/obo/GAZ_00650751">
        <obo:RO_0001025 rdf:resource="http://purl.obolibrary.org/obo/GAZ_00103582"/>
        <obo:IAO_0000115>A lake.</obo:IAO_0000115>
        <oboInOwl:hasOBONamespace>GAZ</oboInOwl:hasOBONamespace>
        <oboInOwl:id>GAZ:00650751</oboInOwl:id>
        <rdfs:label>Tappenkarsee</rdfs:label>
    </owl:NamedIndividual>
    


    <!-- http://purl.obolibrary.org/obo/GAZ_00650758 -->

    <owl:NamedIndividual rdf:about="http://purl.obolibrary.org/obo/GAZ_00650758">
        <rdf:type rdf:resource="http://purl.obolibrary.org/obo/ENVO_00000029"/>
        <obo:RO_0001025 rdf:resource="http://purl.obolibrary.org/obo/GAZ_00650467"/>
        <obo:IAO_0000115>A ravine.</obo:IAO_0000115>
        <oboInOwl:hasOBONamespace>GAZ</oboInOwl:hasOBONamespace>
        <oboInOwl:id>GAZ:00650758</oboInOwl:id>
        <rdfs:label>Seisenbergklamm</rdfs:label>
    </owl:NamedIndividual>
    


    <!-- http://purl.obolibrary.org/obo/GAZ_00650773 -->

    <owl:NamedIndividual rdf:about="http://purl.obolibrary.org/obo/GAZ_00650773">
        <obo:IAO_0000115>A river.</obo:IAO_0000115>
        <oboInOwl:hasOBONamespace>GAZ</oboInOwl:hasOBONamespace>
        <oboInOwl:id>GAZ:00650773</oboInOwl:id>
        <rdfs:label>Selbach</rdfs:label>
    </owl:NamedIndividual>
    


    <!-- http://purl.obolibrary.org/obo/GAZ_00650774 -->

    <owl:NamedIndividual rdf:about="http://purl.obolibrary.org/obo/GAZ_00650774">
        <obo:IAO_0000115>A river.</obo:IAO_0000115>
        <oboInOwl:hasOBONamespace>GAZ</oboInOwl:hasOBONamespace>
        <oboInOwl:id>GAZ:00650774</oboInOwl:id>
        <rdfs:label>Weidebach</rdfs:label>
    </owl:NamedIndividual>
    


    <!-- http://purl.obolibrary.org/obo/GAZ_00650775 -->

    <owl:NamedIndividual rdf:about="http://purl.obolibrary.org/obo/GAZ_00650775">
        <obo:IAO_0000115>A river.</obo:IAO_0000115>
        <oboInOwl:hasOBONamespace>GAZ</oboInOwl:hasOBONamespace>
        <oboInOwl:id>GAZ:00650775</oboInOwl:id>
        <rdfs:label>Lauter</rdfs:label>
    </owl:NamedIndividual>
    


    <!-- http://purl.obolibrary.org/obo/GAZ_00650776 -->

    <owl:NamedIndividual rdf:about="http://purl.obolibrary.org/obo/GAZ_00650776">
        <obo:IAO_0000115>A river.</obo:IAO_0000115>
        <oboInOwl:hasOBONamespace>GAZ</oboInOwl:hasOBONamespace>
        <oboInOwl:id>GAZ:00650776</oboInOwl:id>
        <rdfs:label>Merlachbach</rdfs:label>
    </owl:NamedIndividual>
    


    <!-- http://purl.obolibrary.org/obo/GAZ_00650777 -->

    <owl:NamedIndividual rdf:about="http://purl.obolibrary.org/obo/GAZ_00650777">
        <obo:IAO_0000115>A river.</obo:IAO_0000115>
        <oboInOwl:hasOBONamespace>GAZ</oboInOwl:hasOBONamespace>
        <oboInOwl:id>GAZ:00650777</oboInOwl:id>
        <rdfs:label>Laubach</rdfs:label>
    </owl:NamedIndividual>
    


    <!-- http://purl.obolibrary.org/obo/GAZ_00650782 -->

    <owl:NamedIndividual rdf:about="http://purl.obolibrary.org/obo/GAZ_00650782">
        <obo:IAO_0000115>A river.</obo:IAO_0000115>
        <oboInOwl:hasOBONamespace>GAZ</oboInOwl:hasOBONamespace>
        <oboInOwl:id>GAZ:00650782</oboInOwl:id>
        <rdfs:label>Glasbach</rdfs:label>
    </owl:NamedIndividual>
    


    <!-- http://purl.obolibrary.org/obo/GAZ_00650783 -->

    <owl:NamedIndividual rdf:about="http://purl.obolibrary.org/obo/GAZ_00650783">
        <obo:IAO_0000115>A river.</obo:IAO_0000115>
        <oboInOwl:hasOBONamespace>GAZ</oboInOwl:hasOBONamespace>
        <oboInOwl:id>GAZ:00650783</oboInOwl:id>
        <rdfs:label>Hallwasser</rdfs:label>
    </owl:NamedIndividual>
    


    <!-- http://purl.obolibrary.org/obo/GAZ_00650784 -->

    <owl:NamedIndividual rdf:about="http://purl.obolibrary.org/obo/GAZ_00650784">
        <obo:IAO_0000115>A river.</obo:IAO_0000115>
        <oboInOwl:hasOBONamespace>GAZ</oboInOwl:hasOBONamespace>
        <oboInOwl:id>GAZ:00650784</oboInOwl:id>
        <rdfs:label>Meilschnitz</rdfs:label>
    </owl:NamedIndividual>
    


    <!-- http://purl.obolibrary.org/obo/GAZ_00650785 -->

    <owl:NamedIndividual rdf:about="http://purl.obolibrary.org/obo/GAZ_00650785">
        <obo:IAO_0000115>A river.</obo:IAO_0000115>
        <oboInOwl:hasOBONamespace>GAZ</oboInOwl:hasOBONamespace>
        <oboInOwl:id>GAZ:00650785</oboInOwl:id>
        <rdfs:label>Rottenbachgraben</rdfs:label>
    </owl:NamedIndividual>
    


    <!-- http://purl.obolibrary.org/obo/GAZ_00650786 -->

    <owl:NamedIndividual rdf:about="http://purl.obolibrary.org/obo/GAZ_00650786">
        <obo:IAO_0000115>A river.</obo:IAO_0000115>
        <oboInOwl:hasOBONamespace>GAZ</oboInOwl:hasOBONamespace>
        <oboInOwl:id>GAZ:00650786</oboInOwl:id>
        <rdfs:label>Neuwiesengraben</rdfs:label>
    </owl:NamedIndividual>
    


    <!-- http://purl.obolibrary.org/obo/GAZ_00650787 -->

    <owl:NamedIndividual rdf:about="http://purl.obolibrary.org/obo/GAZ_00650787">
        <obo:IAO_0000115>A river.</obo:IAO_0000115>
        <oboInOwl:hasOBONamespace>GAZ</oboInOwl:hasOBONamespace>
        <oboInOwl:id>GAZ:00650787</oboInOwl:id>
        <rdfs:label>Kemmatener Graben</rdfs:label>
    </owl:NamedIndividual>
    


    <!-- http://purl.obolibrary.org/obo/GAZ_00650788 -->

    <owl:NamedIndividual rdf:about="http://purl.obolibrary.org/obo/GAZ_00650788">
        <obo:IAO_0000115>A river.</obo:IAO_0000115>
        <oboInOwl:hasOBONamespace>GAZ</oboInOwl:hasOBONamespace>
        <oboInOwl:id>GAZ:00650788</oboInOwl:id>
        <rdfs:label>Kehlgraben</rdfs:label>
    </owl:NamedIndividual>
    


    <!-- http://purl.obolibrary.org/obo/GAZ_00650789 -->

    <owl:NamedIndividual rdf:about="http://purl.obolibrary.org/obo/GAZ_00650789">
        <obo:IAO_0000115>A river.</obo:IAO_0000115>
        <oboInOwl:hasOBONamespace>GAZ</oboInOwl:hasOBONamespace>
        <oboInOwl:id>GAZ:00650789</oboInOwl:id>
        <rdfs:label>Stammbachsgraben</rdfs:label>
    </owl:NamedIndividual>
    


    <!-- http://purl.obolibrary.org/obo/GAZ_00650952 -->

    <owl:NamedIndividual rdf:about="http://purl.obolibrary.org/obo/GAZ_00650952">
        <obo:IAO_0000115>A karst spring.</obo:IAO_0000115>
        <oboInOwl:hasOBONamespace>GAZ</oboInOwl:hasOBONamespace>
        <oboInOwl:id>GAZ:00650952</oboInOwl:id>
        <rdfs:label>Karstquelle Hofheim</rdfs:label>
    </owl:NamedIndividual>
    


    <!-- http://purl.obolibrary.org/obo/GAZ_00651039 -->

    <owl:NamedIndividual rdf:about="http://purl.obolibrary.org/obo/GAZ_00651039">
        <obo:IAO_0000115>A headwater of the Rodach.</obo:IAO_0000115>
        <oboInOwl:hasOBONamespace>GAZ</oboInOwl:hasOBONamespace>
        <oboInOwl:id>GAZ:00651039</oboInOwl:id>
        <rdfs:label>Zahme Rodach</rdfs:label>
    </owl:NamedIndividual>
    


    <!-- http://purl.obolibrary.org/obo/GAZ_00651135 -->

    <owl:NamedIndividual rdf:about="http://purl.obolibrary.org/obo/GAZ_00651135">
        <obo:IAO_0000115>A hydroelectric power station.</obo:IAO_0000115>
        <oboInOwl:hasOBONamespace>GAZ</oboInOwl:hasOBONamespace>
        <oboInOwl:id>GAZ:00651135</oboInOwl:id>
        <rdfs:label>Wasserkraftwerk Muhltal</rdfs:label>
    </owl:NamedIndividual>
    


    <!-- http://purl.obolibrary.org/obo/GAZ_00653551 -->

    <owl:NamedIndividual rdf:about="http://purl.obolibrary.org/obo/GAZ_00653551">
        <obo:IAO_0000115>A harbor.</obo:IAO_0000115>
        <oboInOwl:hasOBONamespace>GAZ</oboInOwl:hasOBONamespace>
        <oboInOwl:id>GAZ:00653551</oboInOwl:id>
        <rdfs:label>Hafen Mainkur</rdfs:label>
    </owl:NamedIndividual>
    


    <!-- http://purl.obolibrary.org/obo/GAZ_00653552 -->

    <owl:NamedIndividual rdf:about="http://purl.obolibrary.org/obo/GAZ_00653552">
        <obo:IAO_0000115>A harbor.</obo:IAO_0000115>
        <oboInOwl:hasOBONamespace>GAZ</oboInOwl:hasOBONamespace>
        <oboInOwl:id>GAZ:00653552</oboInOwl:id>
        <rdfs:label>Frankfurter Osthafen</rdfs:label>
    </owl:NamedIndividual>
    


    <!-- http://purl.obolibrary.org/obo/GAZ_00653553 -->

    <owl:NamedIndividual rdf:about="http://purl.obolibrary.org/obo/GAZ_00653553">
        <obo:RO_0001025 rdf:resource="http://purl.obolibrary.org/obo/GAZ_00653552"/>
        <obo:IAO_0000115>A harbor.</obo:IAO_0000115>
        <oboInOwl:hasOBONamespace>GAZ</oboInOwl:hasOBONamespace>
        <oboInOwl:id>GAZ:00653553</oboInOwl:id>
        <rdfs:label>Osthafen - Oberhafen</rdfs:label>
    </owl:NamedIndividual>
    


    <!-- http://purl.obolibrary.org/obo/GAZ_00653554 -->

    <owl:NamedIndividual rdf:about="http://purl.obolibrary.org/obo/GAZ_00653554">
        <obo:RO_0001025 rdf:resource="http://purl.obolibrary.org/obo/GAZ_00653552"/>
        <obo:IAO_0000115>A harbor.</obo:IAO_0000115>
        <oboInOwl:hasOBONamespace>GAZ</oboInOwl:hasOBONamespace>
        <oboInOwl:id>GAZ:00653554</oboInOwl:id>
        <rdfs:label>Osthafen - Unterhafen</rdfs:label>
    </owl:NamedIndividual>
    


    <!-- http://purl.obolibrary.org/obo/GAZ_00653555 -->

    <owl:NamedIndividual rdf:about="http://purl.obolibrary.org/obo/GAZ_00653555">
        <obo:IAO_0000115>A former harbor; now a waterfront.</obo:IAO_0000115>
        <oboInOwl:hasOBONamespace>GAZ</oboInOwl:hasOBONamespace>
        <oboInOwl:id>GAZ:00653555</oboInOwl:id>
        <rdfs:label>Mainkai</rdfs:label>
    </owl:NamedIndividual>
    


    <!-- http://purl.obolibrary.org/obo/GAZ_00653556 -->

    <owl:NamedIndividual rdf:about="http://purl.obolibrary.org/obo/GAZ_00653556">
        <obo:IAO_0000115>A former harbor.</obo:IAO_0000115>
        <oboInOwl:hasOBONamespace>GAZ</oboInOwl:hasOBONamespace>
        <oboInOwl:id>GAZ:00653556</oboInOwl:id>
        <rdfs:label>Schaumainkai</rdfs:label>
    </owl:NamedIndividual>
    


    <!-- http://purl.obolibrary.org/obo/GAZ_00653558 -->

    <owl:NamedIndividual rdf:about="http://purl.obolibrary.org/obo/GAZ_00653558">
        <obo:IAO_0000115>A former harbor.</obo:IAO_0000115>
        <oboInOwl:hasOBONamespace>GAZ</oboInOwl:hasOBONamespace>
        <oboInOwl:id>GAZ:00653558</oboInOwl:id>
        <rdfs:label>Frankfurter Westhafen</rdfs:label>
    </owl:NamedIndividual>
    


    <!-- http://purl.obolibrary.org/obo/GAZ_00653559 -->

    <owl:NamedIndividual rdf:about="http://purl.obolibrary.org/obo/GAZ_00653559">
        <obo:IAO_0000115>A former harbor.</obo:IAO_0000115>
        <oboInOwl:hasOBONamespace>GAZ</oboInOwl:hasOBONamespace>
        <oboInOwl:id>GAZ:00653559</oboInOwl:id>
        <rdfs:label>Hochster Hafen</rdfs:label>
    </owl:NamedIndividual>
    


    <!-- http://purl.obolibrary.org/obo/GAZ_00653579 -->

    <owl:NamedIndividual rdf:about="http://purl.obolibrary.org/obo/GAZ_00653579">
        <obo:RO_0001025 rdf:resource="http://purl.obolibrary.org/obo/GAZ_00653552"/>
        <obo:IAO_0000115>A man-made lake. Formerly part of Frankfurter Osthafen.</obo:IAO_0000115>
        <oboInOwl:hasOBONamespace>GAZ</oboInOwl:hasOBONamespace>
        <oboInOwl:id>GAZ:00653579</oboInOwl:id>
        <rdfs:label>Schwedlersee</rdfs:label>
    </owl:NamedIndividual>
    


    <!-- http://purl.obolibrary.org/obo/GAZ_00653585 -->

    <owl:NamedIndividual rdf:about="http://purl.obolibrary.org/obo/GAZ_00653585">
        <obo:IAO_0000115>A river.</obo:IAO_0000115>
        <oboInOwl:hasOBONamespace>GAZ</oboInOwl:hasOBONamespace>
        <oboInOwl:id>GAZ:00653585</oboInOwl:id>
        <rdfs:label>Gerathsbach</rdfs:label>
    </owl:NamedIndividual>
    


    <!-- http://purl.obolibrary.org/obo/GAZ_00653715 -->

    <owl:NamedIndividual rdf:about="http://purl.obolibrary.org/obo/GAZ_00653715">
        <obo:IAO_0000115>A hydroelectric power station.</obo:IAO_0000115>
        <oboInOwl:hasOBONamespace>GAZ</oboInOwl:hasOBONamespace>
        <oboInOwl:id>GAZ:00653715</oboInOwl:id>
        <rdfs:label>Wasserkraftwerk Dingolfing</rdfs:label>
    </owl:NamedIndividual>
    


    <!-- http://purl.obolibrary.org/obo/GAZ_00653783 -->

    <owl:NamedIndividual rdf:about="http://purl.obolibrary.org/obo/GAZ_00653783">
        <obo:IAO_0000115>A harbor.</obo:IAO_0000115>
        <oboInOwl:hasOBONamespace>GAZ</oboInOwl:hasOBONamespace>
        <oboInOwl:id>GAZ:00653783</oboInOwl:id>
        <rdfs:label>Offenbacher Hafen</rdfs:label>
    </owl:NamedIndividual>
    


    <!-- http://purl.obolibrary.org/obo/GAZ_00653810 -->

    <owl:NamedIndividual rdf:about="http://purl.obolibrary.org/obo/GAZ_00653810">
        <obo:RO_0001025 rdf:resource="http://purl.obolibrary.org/obo/GAZ_00008262"/>
        <obo:IAO_0000115>A harbor.</obo:IAO_0000115>
        <oboInOwl:hasOBONamespace>GAZ</oboInOwl:hasOBONamespace>
        <oboInOwl:id>GAZ:00653810</oboInOwl:id>
        <rdfs:label>Schiersteiner Hafen</rdfs:label>
    </owl:NamedIndividual>
    


    <!-- http://purl.obolibrary.org/obo/GAZ_00654182 -->

    <owl:NamedIndividual rdf:about="http://purl.obolibrary.org/obo/GAZ_00654182">
        <obo:IAO_0000115>A river.</obo:IAO_0000115>
        <oboInOwl:hasOBONamespace>GAZ</oboInOwl:hasOBONamespace>
        <oboInOwl:id>GAZ:00654182</oboInOwl:id>
        <rdfs:label>Wurf</rdfs:label>
    </owl:NamedIndividual>
    


    <!-- http://purl.obolibrary.org/obo/GAZ_00654185 -->

    <owl:NamedIndividual rdf:about="http://purl.obolibrary.org/obo/GAZ_00654185">
        <obo:IAO_0000115>A river.</obo:IAO_0000115>
        <oboInOwl:hasOBONamespace>GAZ</oboInOwl:hasOBONamespace>
        <oboInOwl:id>GAZ:00654185</oboInOwl:id>
        <rdfs:label>Wohlgraben</rdfs:label>
    </owl:NamedIndividual>
    


    <!-- http://purl.obolibrary.org/obo/GAZ_00654327 -->

    <owl:NamedIndividual rdf:about="http://purl.obolibrary.org/obo/GAZ_00654327">
        <obo:IAO_0000115>A reservoir, It is between Mademuhlen und Driedorf im Westerwald.</obo:IAO_0000115>
        <oboInOwl:hasOBONamespace>GAZ</oboInOwl:hasOBONamespace>
        <oboInOwl:id>GAZ:00654327</oboInOwl:id>
        <rdfs:label>Stausee Driedorf</rdfs:label>
    </owl:NamedIndividual>
    


    <!-- http://purl.obolibrary.org/obo/GAZ_00654328 -->

    <owl:NamedIndividual rdf:about="http://purl.obolibrary.org/obo/GAZ_00654328">
        <obo:IAO_0000115>A dam.</obo:IAO_0000115>
        <oboInOwl:hasOBONamespace>GAZ</oboInOwl:hasOBONamespace>
        <oboInOwl:id>GAZ:00654328</oboInOwl:id>
        <rdfs:label>Krombachtalsperre</rdfs:label>
    </owl:NamedIndividual>
    


    <!-- http://purl.obolibrary.org/obo/GAZ_00654329 -->

    <owl:NamedIndividual rdf:about="http://purl.obolibrary.org/obo/GAZ_00654329">
        <obo:IAO_0000115>A reservoir; held by the Krombachtalsperre.</obo:IAO_0000115>
        <oboInOwl:hasOBONamespace>GAZ</oboInOwl:hasOBONamespace>
        <oboInOwl:id>GAZ:00654329</oboInOwl:id>
        <rdfs:label>Krombachstausee</rdfs:label>
    </owl:NamedIndividual>
    


    <!-- http://purl.obolibrary.org/obo/GAZ_00654368 -->

    <owl:NamedIndividual rdf:about="http://purl.obolibrary.org/obo/GAZ_00654368">
        <obo:IAO_0000115>A flood control reservoir.</obo:IAO_0000115>
        <oboInOwl:hasOBONamespace>GAZ</oboInOwl:hasOBONamespace>
        <oboInOwl:id>GAZ:00654368</oboInOwl:id>
        <rdfs:label>Ulmbachtalsperre</rdfs:label>
    </owl:NamedIndividual>
    


    <!-- http://purl.obolibrary.org/obo/GAZ_00654562 -->

    <owl:NamedIndividual rdf:about="http://purl.obolibrary.org/obo/GAZ_00654562">
        <obo:RO_0001025 rdf:resource="http://purl.obolibrary.org/obo/GAZ_00008262"/>
        <obo:IAO_0000115>A harbor.</obo:IAO_0000115>
        <oboInOwl:hasOBONamespace>GAZ</oboInOwl:hasOBONamespace>
        <oboInOwl:id>GAZ:00654562</oboInOwl:id>
        <rdfs:label>Gernsheimer Hafen</rdfs:label>
    </owl:NamedIndividual>
    


    <!-- http://purl.obolibrary.org/obo/GAZ_00654563 -->

    <owl:NamedIndividual rdf:about="http://purl.obolibrary.org/obo/GAZ_00654563">
        <obo:RO_0001025 rdf:resource="http://purl.obolibrary.org/obo/GAZ_00008262"/>
        <obo:IAO_0000115>A harbor.</obo:IAO_0000115>
        <oboInOwl:hasOBONamespace>GAZ</oboInOwl:hasOBONamespace>
        <oboInOwl:id>GAZ:00654563</oboInOwl:id>
        <rdfs:label>Gernsheimer Containerhafen</rdfs:label>
    </owl:NamedIndividual>
    


    <!-- http://purl.obolibrary.org/obo/GAZ_00655231 -->

    <owl:NamedIndividual rdf:about="http://purl.obolibrary.org/obo/GAZ_00655231">
        <rdf:type rdf:resource="http://purl.obolibrary.org/obo/ENVO_00000423"/>
        <obo:RO_0001025 rdf:resource="http://purl.obolibrary.org/obo/GAZ_00008262"/>
        <obo:IAO_0000115>A fluvial island.</obo:IAO_0000115>
        <oboInOwl:hasOBONamespace>GAZ</oboInOwl:hasOBONamespace>
        <oboInOwl:id>GAZ:00655231</oboInOwl:id>
        <rdfs:label>Mariannenaue</rdfs:label>
    </owl:NamedIndividual>
    


    <!-- http://purl.obolibrary.org/obo/GAZ_00655646 -->

    <owl:NamedIndividual rdf:about="http://purl.obolibrary.org/obo/GAZ_00655646">
        <obo:IAO_0000115>A dam.</obo:IAO_0000115>
        <oboInOwl:hasOBONamespace>GAZ</oboInOwl:hasOBONamespace>
        <oboInOwl:id>GAZ:00655646</oboInOwl:id>
        <rdfs:label>Aartalsperre</rdfs:label>
    </owl:NamedIndividual>
    


    <!-- http://purl.obolibrary.org/obo/GAZ_00655647 -->

    <owl:NamedIndividual rdf:about="http://purl.obolibrary.org/obo/GAZ_00655647">
        <obo:IAO_0000115>A man-made lake created by the Aartalsperre.</obo:IAO_0000115>
        <oboInOwl:hasOBONamespace>GAZ</oboInOwl:hasOBONamespace>
        <oboInOwl:id>GAZ:00655647</oboInOwl:id>
        <rdfs:label>Aartalsee</rdfs:label>
    </owl:NamedIndividual>
    


    <!-- http://purl.obolibrary.org/obo/GAZ_00655832 -->

    <owl:NamedIndividual rdf:about="http://purl.obolibrary.org/obo/GAZ_00655832">
        <obo:IAO_0000115>A drinking water reservoir.</obo:IAO_0000115>
        <oboInOwl:hasOBONamespace>GAZ</oboInOwl:hasOBONamespace>
        <oboInOwl:id>GAZ:00655832</oboInOwl:id>
        <rdfs:label>Genkeltalsperre</rdfs:label>
    </owl:NamedIndividual>
    


    <!-- http://purl.obolibrary.org/obo/GAZ_00655842 -->

    <owl:NamedIndividual rdf:about="http://purl.obolibrary.org/obo/GAZ_00655842">
        <obo:IAO_0000115>A drinking water reservoir.</obo:IAO_0000115>
        <oboInOwl:hasOBONamespace>GAZ</oboInOwl:hasOBONamespace>
        <oboInOwl:id>GAZ:00655842</oboInOwl:id>
        <rdfs:label>Wiehltalsperre</rdfs:label>
    </owl:NamedIndividual>
    


    <!-- http://purl.obolibrary.org/obo/GAZ_00655911 -->

    <owl:NamedIndividual rdf:about="http://purl.obolibrary.org/obo/GAZ_00655911">
        <obo:IAO_0000115>A river.</obo:IAO_0000115>
        <oboInOwl:hasOBONamespace>GAZ</oboInOwl:hasOBONamespace>
        <oboInOwl:id>GAZ:00655911</oboInOwl:id>
        <rdfs:label>Olpebach</rdfs:label>
    </owl:NamedIndividual>
    


    <!-- http://purl.obolibrary.org/obo/GAZ_00655912 -->

    <owl:NamedIndividual rdf:about="http://purl.obolibrary.org/obo/GAZ_00655912">
        <obo:IAO_0000115>A river.</obo:IAO_0000115>
        <oboInOwl:hasOBONamespace>GAZ</oboInOwl:hasOBONamespace>
        <oboInOwl:id>GAZ:00655912</oboInOwl:id>
        <rdfs:label>Altenbach</rdfs:label>
    </owl:NamedIndividual>
    


    <!-- http://purl.obolibrary.org/obo/GAZ_00655913 -->

    <owl:NamedIndividual rdf:about="http://purl.obolibrary.org/obo/GAZ_00655913">
        <obo:IAO_0000115>A river.</obo:IAO_0000115>
        <oboInOwl:hasOBONamespace>GAZ</oboInOwl:hasOBONamespace>
        <oboInOwl:id>GAZ:00655913</oboInOwl:id>
        <rdfs:label>Dahlbach</rdfs:label>
    </owl:NamedIndividual>
    


    <!-- http://purl.obolibrary.org/obo/GAZ_00655914 -->

    <owl:NamedIndividual rdf:about="http://purl.obolibrary.org/obo/GAZ_00655914">
        <obo:IAO_0000115>A river.</obo:IAO_0000115>
        <oboInOwl:hasOBONamespace>GAZ</oboInOwl:hasOBONamespace>
        <oboInOwl:id>GAZ:00655914</oboInOwl:id>
        <rdfs:label>Schwarzenbach</rdfs:label>
    </owl:NamedIndividual>
    


    <!-- http://purl.obolibrary.org/obo/GAZ_00655915 -->

    <owl:NamedIndividual rdf:about="http://purl.obolibrary.org/obo/GAZ_00655915">
        <obo:IAO_0000115>A river.</obo:IAO_0000115>
        <oboInOwl:hasOBONamespace>GAZ</oboInOwl:hasOBONamespace>
        <oboInOwl:id>GAZ:00655915</oboInOwl:id>
        <rdfs:label>Flosbach</rdfs:label>
    </owl:NamedIndividual>
    


    <!-- http://purl.obolibrary.org/obo/GAZ_00655916 -->

    <owl:NamedIndividual rdf:about="http://purl.obolibrary.org/obo/GAZ_00655916">
        <obo:IAO_0000115>A river.</obo:IAO_0000115>
        <oboInOwl:hasOBONamespace>GAZ</oboInOwl:hasOBONamespace>
        <oboInOwl:id>GAZ:00655916</oboInOwl:id>
        <rdfs:label>Drecker Bach</rdfs:label>
    </owl:NamedIndividual>
    


    <!-- http://purl.obolibrary.org/obo/GAZ_00655937 -->

    <owl:NamedIndividual rdf:about="http://purl.obolibrary.org/obo/GAZ_00655937">
        <obo:IAO_0000115>A dam; forms the Obernaustausee.</obo:IAO_0000115>
        <oboInOwl:hasOBONamespace>GAZ</oboInOwl:hasOBONamespace>
        <oboInOwl:id>GAZ:00655937</oboInOwl:id>
        <rdfs:label>Obernautalsperre</rdfs:label>
    </owl:NamedIndividual>
    


    <!-- http://purl.obolibrary.org/obo/GAZ_00658513 -->

    <owl:NamedIndividual rdf:about="http://purl.obolibrary.org/obo/GAZ_00658513">
        <obo:IAO_0000115>A lake.</obo:IAO_0000115>
        <oboInOwl:hasOBONamespace>GAZ</oboInOwl:hasOBONamespace>
        <oboInOwl:id>GAZ:00658513</oboInOwl:id>
        <rdfs:label>Oberjgermeisterteich</rdfs:label>
    </owl:NamedIndividual>
    


    <!-- http://purl.obolibrary.org/obo/GAZ_00658591 -->

    <owl:NamedIndividual rdf:about="http://purl.obolibrary.org/obo/GAZ_00658591">
        <obo:IAO_0000115>A lake.</obo:IAO_0000115>
        <oboInOwl:hasOBONamespace>GAZ</oboInOwl:hasOBONamespace>
        <oboInOwl:id>GAZ:00658591</oboInOwl:id>
        <rdfs:label>Wispersee</rdfs:label>
    </owl:NamedIndividual>
    


    <!-- http://purl.obolibrary.org/obo/GAZ_00658605 -->

    <owl:NamedIndividual rdf:about="http://purl.obolibrary.org/obo/GAZ_00658605">
        <obo:IAO_0000115>A river,</obo:IAO_0000115>
        <oboInOwl:hasOBONamespace>GAZ</oboInOwl:hasOBONamespace>
        <oboInOwl:id>GAZ:00658605</oboInOwl:id>
        <rdfs:label>Galgenbach $$$</rdfs:label>
    </owl:NamedIndividual>
    


    <!-- http://purl.obolibrary.org/obo/GAZ_00658606 -->

    <owl:NamedIndividual rdf:about="http://purl.obolibrary.org/obo/GAZ_00658606">
        <oboInOwl:hasOBONamespace>GAZ</oboInOwl:hasOBONamespace>
        <oboInOwl:id>GAZ:00658606</oboInOwl:id>
        <rdfs:label>Weilbach</rdfs:label>
    </owl:NamedIndividual>
    


    <!-- http://purl.obolibrary.org/obo/GAZ_00658620 -->

    <owl:NamedIndividual rdf:about="http://purl.obolibrary.org/obo/GAZ_00658620">
        <obo:IAO_0000115>A river.</obo:IAO_0000115>
        <oboInOwl:hasOBONamespace>GAZ</oboInOwl:hasOBONamespace>
        <oboInOwl:id>GAZ:00658620</oboInOwl:id>
        <rdfs:label>Mhlborn$$$</rdfs:label>
    </owl:NamedIndividual>
    


    <!-- http://purl.obolibrary.org/obo/GAZ_00658621 -->

    <owl:NamedIndividual rdf:about="http://purl.obolibrary.org/obo/GAZ_00658621">
        <oboInOwl:hasOBONamespace>GAZ</oboInOwl:hasOBONamespace>
        <oboInOwl:id>GAZ:00658621</oboInOwl:id>
        <rdfs:label>Sangeborn</rdfs:label>
    </owl:NamedIndividual>
    


    <!-- http://purl.obolibrary.org/obo/GAZ_00658622 -->

    <owl:NamedIndividual rdf:about="http://purl.obolibrary.org/obo/GAZ_00658622">
        <oboInOwl:hasOBONamespace>GAZ</oboInOwl:hasOBONamespace>
        <oboInOwl:id>GAZ:00658622</oboInOwl:id>
        <rdfs:label>Lotzengrundbach</rdfs:label>
    </owl:NamedIndividual>
    


    <!-- http://purl.obolibrary.org/obo/GAZ_00658623 -->

    <owl:NamedIndividual rdf:about="http://purl.obolibrary.org/obo/GAZ_00658623">
        <oboInOwl:hasOBONamespace>GAZ</oboInOwl:hasOBONamespace>
        <oboInOwl:id>GAZ:00658623</oboInOwl:id>
        <rdfs:label>Bach von der Goldgrube</rdfs:label>
    </owl:NamedIndividual>
    


    <!-- http://purl.obolibrary.org/obo/GAZ_00658629 -->

    <owl:NamedIndividual rdf:about="http://purl.obolibrary.org/obo/GAZ_00658629">
        <obo:IAO_0000115>A river.</obo:IAO_0000115>
        <oboInOwl:hasOBONamespace>GAZ</oboInOwl:hasOBONamespace>
        <oboInOwl:id>GAZ:00658629</oboInOwl:id>
        <rdfs:label>Markbach  $$$</rdfs:label>
    </owl:NamedIndividual>
    


    <!-- http://purl.obolibrary.org/obo/GAZ_00658630 -->

    <owl:NamedIndividual rdf:about="http://purl.obolibrary.org/obo/GAZ_00658630">
        <oboInOwl:hasOBONamespace>GAZ</oboInOwl:hasOBONamespace>
        <oboInOwl:id>GAZ:00658630</oboInOwl:id>
        <rdfs:label>Schmalbach</rdfs:label>
    </owl:NamedIndividual>
    


    <!-- http://purl.obolibrary.org/obo/GAZ_00658669 -->

    <owl:NamedIndividual rdf:about="http://purl.obolibrary.org/obo/GAZ_00658669">
        <obo:IAO_0000115>A reservoir.</obo:IAO_0000115>
        <oboInOwl:hasOBONamespace>GAZ</oboInOwl:hasOBONamespace>
        <oboInOwl:id>GAZ:00658669</oboInOwl:id>
        <rdfs:label>Perfstausee</rdfs:label>
    </owl:NamedIndividual>
    


    <!-- http://purl.obolibrary.org/obo/GAZ_00658686 -->

    <owl:NamedIndividual rdf:about="http://purl.obolibrary.org/obo/GAZ_00658686">
        <obo:IAO_0000115>A lake.</obo:IAO_0000115>
        <oboInOwl:hasOBONamespace>GAZ</oboInOwl:hasOBONamespace>
        <oboInOwl:id>GAZ:00658686</oboInOwl:id>
        <rdfs:label>Spieweiher</rdfs:label>
    </owl:NamedIndividual>
    


    <!-- 
    ///////////////////////////////////////////////////////////////////////////////////////
    //
    // Annotations
    //
    ///////////////////////////////////////////////////////////////////////////////////////
     -->

    <rdf:Description rdf:about="http://purl.obolibrary.org/obo/GAZ_00005367">
        <oboInOwl:hasOBONamespace>GAZ</oboInOwl:hasOBONamespace>
        <rdfs:label>Veere</rdfs:label>
        <oboInOwl:id>GAZ:00005367</oboInOwl:id>
    </rdf:Description>
    <rdf:Description rdf:about="http://purl.obolibrary.org/obo/GAZ_00005544">
        <oboInOwl:hasOBONamespace>GAZ</oboInOwl:hasOBONamespace>
        <rdfs:label>Wilhelminadorp</rdfs:label>
        <oboInOwl:id>GAZ:00005544</oboInOwl:id>
        <obo:IAO_0000115>A populated place.</obo:IAO_0000115>
    </rdf:Description>
    <rdf:Description rdf:about="http://purl.obolibrary.org/obo/GAZ_00007412">
        <oboInOwl:id>GAZ:00007412</oboInOwl:id>
        <rdfs:label>Zwijndrecht</rdfs:label>
        <obo:IAO_0000115>A populated place.</obo:IAO_0000115>
        <oboInOwl:hasOBONamespace>GAZ</oboInOwl:hasOBONamespace>
    </rdf:Description>
    <rdf:Description rdf:about="http://purl.obolibrary.org/obo/GAZ_00008262">
        <rdfs:label>Rhine</rdfs:label>
        <oboInOwl:hasOBONamespace>GAZ</oboInOwl:hasOBONamespace>
        <obo:IAO_0000115>A river that in the Swiss Alps in the canton of Graubunden, where its two main initial tributaries are called Vorderrhein and Hinterrhein. The Vorderrhein (anterior Rhine) springs from Lake Tuma near the Oberalp Pass and passes the impressive Ruinaulta (the Swiss Grand Canyon). The Hinterrhein (posterior Rhine) starts from the Paradies glacier near the Rheinquellhorn at the southern border of Switzerland. One of the latter tributaries originates in Val di Lei in Italy. Both tributaries meet near Reichenau, still in Graubunden. From Reichenau, the Rhine flows north as the Alpenrhein passing Chur and forming the frontier between Liechtenstein and then Austria on the east side, and canton St. Gallen of Switzerland on the west side, then discharging to Lake Constance. Emerging from Lake Constance, flowing generally westward as the Hochrhein it passes the Rhine Falls and is joined by the Aare river which more than doubles its water discharge to an average of nearly 1,000 cubic meters per second. Past Basel, as the Upper Rhine, it forms the southern part of the border between Germany and France in a wide valley, before entering Germany exclusively at Rheinstetten, near Karlsruhe. Between Bingen and Bonn, the Middle Rhine flows through the Rhine Gorge. After crssong the Netherlands border the Rhine turns west and enters the Netherlands, where together with the rivers Meuse and Scheldt it forms the extensive Rhine-Meuse-Scheldt delta, one of the larger river deltas in western Europe. Crossing the border into the Netherlands at Spijk, close to Nijmegen and Arnhem the Rhine is at its widest, but the river then splits into three main distributaries: the Waal, Nederrijn (&quot;Lower Rhine&quot;) and IJssel. From here the situation becomes more complicated, as the Dutch name &quot;Rijn&quot; no longer coincides with the main flow of water. Most of the Rhine water (two thirds) flows farther west through the Waal and then via the Merwede and Nieuwe Merwede (Biesbosch) and, merging with the Meuse, through the Hollands Diep and Haringvliet estuaries into the North Sea. The Beneden Merwede branches off near Hardinxveld-Giessendam and continues as the Noord, to join the Lek near the village of Kinderdijk to form the Nieuwe Maas, then flows past Rotterdam and continues via Het Scheur and the Nieuwe Waterweg to the North Sea. The Oude Maas branches off near Dordrecht, farther down rejoining the Nieuwe Maas to form Het Scheur. The other third portion of the water flows through the Pannerdens Kanaal and redistributes in the IJssel and Nederrijn. The IJssel branch carries one ninth of the water volume north into the IJsselmeer (a former bay), while the Nederrijn flows west parallel to the Waal and carries approximately two ninths of the flow. However, at Wijk bij Duurstede the Nederrijn changes its name and becomes the Lek. It flows farther west to rejoin the Noord into the Nieuwe Maas and to the North Sea.</obo:IAO_0000115>
        <oboInOwl:id>GAZ:00008262</oboInOwl:id>
    </rdf:Description>
    <rdf:Description rdf:about="http://purl.obolibrary.org/obo/GAZ_00009543">
        <oboInOwl:id>GAZ:00009543</oboInOwl:id>
        <rdfs:label>Commune (Liechtenstein)</rdfs:label>
        <oboInOwl:hasOBONamespace>GAZ</oboInOwl:hasOBONamespace>
    </rdf:Description>
    <rdf:Description rdf:about="http://purl.obolibrary.org/obo/GAZ_00013805">
        <rdfs:label>Commune of Gamprin</rdfs:label>
        <obo:IAO_0000115>A municipality.</obo:IAO_0000115>
        <oboInOwl:hasOBONamespace>GAZ</oboInOwl:hasOBONamespace>
        <oboInOwl:id>GAZ:00013805</oboInOwl:id>
    </rdf:Description>
    <rdf:Description rdf:about="http://purl.obolibrary.org/obo/GAZ_00013807">
        <rdfs:label>Commune of Triesen</rdfs:label>
        <obo:IAO_0000115>A municipality.</obo:IAO_0000115>
        <oboInOwl:id>GAZ:00013807</oboInOwl:id>
        <oboInOwl:hasOBONamespace>GAZ</oboInOwl:hasOBONamespace>
    </rdf:Description>
    <rdf:Description rdf:about="http://purl.obolibrary.org/obo/GAZ_00013808">
        <obo:IAO_0000115>A municipality.</obo:IAO_0000115>
        <rdfs:label>Commune of Planken</rdfs:label>
        <oboInOwl:id>GAZ:00013808</oboInOwl:id>
        <oboInOwl:hasOBONamespace>GAZ</oboInOwl:hasOBONamespace>
    </rdf:Description>
    <rdf:Description rdf:about="http://purl.obolibrary.org/obo/GAZ_00013809">
        <obo:IAO_0000115>A municipality.</obo:IAO_0000115>
        <oboInOwl:id>GAZ:00013809</oboInOwl:id>
        <oboInOwl:hasOBONamespace>GAZ</oboInOwl:hasOBONamespace>
        <rdfs:label>Commune of Vaduz</rdfs:label>
    </rdf:Description>
    <rdf:Description rdf:about="http://purl.obolibrary.org/obo/GAZ_00013810">
        <oboInOwl:id>GAZ:00013810</oboInOwl:id>
        <oboInOwl:hasOBONamespace>GAZ</oboInOwl:hasOBONamespace>
        <obo:IAO_0000115>A municipality.</obo:IAO_0000115>
        <rdfs:label>Commune of Ruggell</rdfs:label>
    </rdf:Description>
    <rdf:Description rdf:about="http://purl.obolibrary.org/obo/GAZ_00013811">
        <oboInOwl:hasOBONamespace>GAZ</oboInOwl:hasOBONamespace>
        <obo:IAO_0000115>A municipality.</obo:IAO_0000115>
        <oboInOwl:id>GAZ:00013811</oboInOwl:id>
        <rdfs:label>Commune of Eschen</rdfs:label>
    </rdf:Description>
    <rdf:Description rdf:about="http://purl.obolibrary.org/obo/GAZ_00013812">
        <oboInOwl:id>GAZ:00013812</oboInOwl:id>
        <rdfs:label>Commune of Triesenberg</rdfs:label>
        <obo:IAO_0000115>A municipality.</obo:IAO_0000115>
        <oboInOwl:hasOBONamespace>GAZ</oboInOwl:hasOBONamespace>
    </rdf:Description>
    <rdf:Description rdf:about="http://purl.obolibrary.org/obo/GAZ_00013813">
        <oboInOwl:id>GAZ:00013813</oboInOwl:id>
        <oboInOwl:hasOBONamespace>GAZ</oboInOwl:hasOBONamespace>
        <obo:IAO_0000115>A municipality.</obo:IAO_0000115>
        <rdfs:label>Commune of Schellenberg</rdfs:label>
    </rdf:Description>
    <rdf:Description rdf:about="http://purl.obolibrary.org/obo/GAZ_00013814">
        <oboInOwl:id>GAZ:00013814</oboInOwl:id>
        <rdfs:label>Commune of Mauren</rdfs:label>
        <obo:IAO_0000115>A municipality.</obo:IAO_0000115>
        <oboInOwl:hasOBONamespace>GAZ</oboInOwl:hasOBONamespace>
    </rdf:Description>
    <rdf:Description rdf:about="http://purl.obolibrary.org/obo/GAZ_00013815">
        <oboInOwl:id>GAZ:00013815</oboInOwl:id>
        <rdfs:label>Commune of Balzers</rdfs:label>
        <obo:IAO_0000115>A municipality.</obo:IAO_0000115>
        <oboInOwl:hasOBONamespace>GAZ</oboInOwl:hasOBONamespace>
    </rdf:Description>
    <rdf:Description rdf:about="http://purl.obolibrary.org/obo/GAZ_00013816">
        <rdfs:label>Schaanwald</rdfs:label>
        <oboInOwl:hasOBONamespace>GAZ</oboInOwl:hasOBONamespace>
        <oboInOwl:id>GAZ:00013816</oboInOwl:id>
        <obo:IAO_0000115>A populated place.</obo:IAO_0000115>
    </rdf:Description>
    <rdf:Description rdf:about="http://purl.obolibrary.org/obo/GAZ_00013817">
        <oboInOwl:hasOBONamespace>GAZ</oboInOwl:hasOBONamespace>
        <rdfs:label>populated place, Liechtenstein</rdfs:label>
        <oboInOwl:id>GAZ:00013817</oboInOwl:id>
    </rdf:Description>
    <rdf:Description rdf:about="http://purl.obolibrary.org/obo/GAZ_00060232">
        <oboInOwl:hasOBONamespace>GAZ</oboInOwl:hasOBONamespace>
        <oboInOwl:id>GAZ:00060232</oboInOwl:id>
        <obo:IAO_0000115>Lakes in the Queyras Valley.</obo:IAO_0000115>
        <rdfs:label>Lacs Guil-Agnelle</rdfs:label>
    </rdf:Description>
    <rdf:Description rdf:about="http://purl.obolibrary.org/obo/GAZ_00060233">
        <rdfs:label>Lacs du Guil</rdfs:label>
        <oboInOwl:hasOBONamespace>GAZ</oboInOwl:hasOBONamespace>
        <oboInOwl:id>GAZ:00060233</oboInOwl:id>
        <obo:IAO_0000115>Lakes in the Queyras Valley.</obo:IAO_0000115>
    </rdf:Description>
    <rdf:Description rdf:about="http://purl.obolibrary.org/obo/GAZ_00060240">
        <oboInOwl:id>GAZ:00060240</oboInOwl:id>
        <oboInOwl:hasOBONamespace>GAZ</oboInOwl:hasOBONamespace>
        <obo:IAO_0000115>Lakes in the Queyras Valley.</obo:IAO_0000115>
        <rdfs:label>Lacs du Malrif</rdfs:label>
    </rdf:Description>
    <rdf:Description rdf:about="http://purl.obolibrary.org/obo/GAZ_00060404">
        <obo:IAO_0000115>A group of lakes (though &gt;7) in La chaine de Belledonne at 2248m.</obo:IAO_0000115>
        <oboInOwl:id>GAZ:00060404</oboInOwl:id>
        <rdfs:label>Sept Laux</rdfs:label>
        <oboInOwl:hasOBONamespace>GAZ</oboInOwl:hasOBONamespace>
    </rdf:Description>
    <rdf:Description rdf:about="http://purl.obolibrary.org/obo/GAZ_00060410">
        <obo:IAO_0000115>A lake in La chaine de Belledonne.</obo:IAO_0000115>
        <rdfs:label>Lac du Cos</rdfs:label>
        <oboInOwl:hasOBONamespace>GAZ</oboInOwl:hasOBONamespace>
        <oboInOwl:id>GAZ:00060410</oboInOwl:id>
    </rdf:Description>
    <rdf:Description rdf:about="http://purl.obolibrary.org/obo/GAZ_00619830">
        <rdfs:label>Isar-werk Kanal</rdfs:label>
        <obo:IAO_0000115>A river.</obo:IAO_0000115>
        <oboInOwl:id>GAZ:00619830</oboInOwl:id>
        <oboInOwl:hasOBONamespace>GAZ</oboInOwl:hasOBONamespace>
    </rdf:Description>
</rdf:RDF>



<!-- Generated by the OWL API (version 4.5.6) https://github.com/owlcs/owlapi -->

