<?xml version="1.0"?>
<rdf:RDF xmlns="http://purl.obolibrary.org/obo/gaz/subsets/countries/Madagascar.owl#"
     xml:base="http://purl.obolibrary.org/obo/gaz/subsets/countries/Madagascar.owl"
     xmlns:obo="http://purl.obolibrary.org/obo/"
     xmlns:owl="http://www.w3.org/2002/07/owl#"
     xmlns:rdf="http://www.w3.org/1999/02/22-rdf-syntax-ns#"
     xmlns:xml="http://www.w3.org/XML/1998/namespace"
     xmlns:xsd="http://www.w3.org/2001/XMLSchema#"
     xmlns:rdfs="http://www.w3.org/2000/01/rdf-schema#"
     xmlns:oboInOwl="http://www.geneontology.org/formats/oboInOwl#">
    <owl:Ontology rdf:about="http://purl.obolibrary.org/obo/gaz/subsets/countries/Madagascar.owl">
        <owl:imports rdf:resource="http://purl.obolibrary.org/obo/gaz/imports/envo_import.owl"/>
        <owl:imports rdf:resource="http://purl.obolibrary.org/obo/gaz/imports/ro_import.owl"/>
    </owl:Ontology>
    


    <!-- 
    ///////////////////////////////////////////////////////////////////////////////////////
    //
    // Annotation properties
    //
    ///////////////////////////////////////////////////////////////////////////////////////
     -->

    


    <!-- http://purl.obolibrary.org/obo/IAO_0000115 -->

    <owl:AnnotationProperty rdf:about="http://purl.obolibrary.org/obo/IAO_0000115"/>
    


    <!-- http://www.geneontology.org/formats/oboInOwl#hasOBONamespace -->

    <owl:AnnotationProperty rdf:about="http://www.geneontology.org/formats/oboInOwl#hasOBONamespace"/>
    


    <!-- http://www.geneontology.org/formats/oboInOwl#id -->

    <owl:AnnotationProperty rdf:about="http://www.geneontology.org/formats/oboInOwl#id"/>
    


    <!-- 
    ///////////////////////////////////////////////////////////////////////////////////////
    //
    // Object Properties
    //
    ///////////////////////////////////////////////////////////////////////////////////////
     -->

    


    <!-- http://purl.obolibrary.org/obo/RO_0001025 -->

    <owl:ObjectProperty rdf:about="http://purl.obolibrary.org/obo/RO_0001025"/>
    


    <!-- 
    ///////////////////////////////////////////////////////////////////////////////////////
    //
    // Classes
    //
    ///////////////////////////////////////////////////////////////////////////////////////
     -->

    


    <!-- http://purl.obolibrary.org/obo/ENVO_00000004 -->

    <owl:Class rdf:about="http://purl.obolibrary.org/obo/ENVO_00000004"/>
    


    <!-- http://purl.obolibrary.org/obo/ENVO_00000222 -->

    <owl:Class rdf:about="http://purl.obolibrary.org/obo/ENVO_00000222"/>
    


    <!-- http://purl.obolibrary.org/obo/ENVO_00000856 -->

    <owl:Class rdf:about="http://purl.obolibrary.org/obo/ENVO_00000856"/>
    


    <!-- http://purl.obolibrary.org/obo/GAZ_00005421 -->

    <owl:Class rdf:about="http://purl.obolibrary.org/obo/GAZ_00005421"/>
    


    <!-- http://purl.obolibrary.org/obo/GAZ_00005422 -->

    <owl:Class rdf:about="http://purl.obolibrary.org/obo/GAZ_00005422">
        <rdfs:subClassOf rdf:resource="http://purl.obolibrary.org/obo/GAZ_00005421"/>
    </owl:Class>
    


    <!-- http://purl.obolibrary.org/obo/GAZ_00005423 -->

    <owl:Class rdf:about="http://purl.obolibrary.org/obo/GAZ_00005423">
        <rdfs:subClassOf rdf:resource="http://purl.obolibrary.org/obo/GAZ_00005421"/>
    </owl:Class>
    


    <!-- http://purl.obolibrary.org/obo/GAZ_00005424 -->

    <owl:Class rdf:about="http://purl.obolibrary.org/obo/GAZ_00005424">
        <rdfs:subClassOf rdf:resource="http://purl.obolibrary.org/obo/GAZ_00005421"/>
    </owl:Class>
    


    <!-- http://purl.obolibrary.org/obo/GAZ_00005425 -->

    <owl:Class rdf:about="http://purl.obolibrary.org/obo/GAZ_00005425">
        <rdfs:subClassOf rdf:resource="http://purl.obolibrary.org/obo/GAZ_00005421"/>
    </owl:Class>
    


    <!-- http://purl.obolibrary.org/obo/GAZ_00005426 -->

    <owl:Class rdf:about="http://purl.obolibrary.org/obo/GAZ_00005426">
        <rdfs:subClassOf rdf:resource="http://purl.obolibrary.org/obo/GAZ_00005421"/>
    </owl:Class>
    


    <!-- http://purl.obolibrary.org/obo/GAZ_00005427 -->

    <owl:Class rdf:about="http://purl.obolibrary.org/obo/GAZ_00005427">
        <rdfs:subClassOf rdf:resource="http://purl.obolibrary.org/obo/GAZ_00005421"/>
    </owl:Class>
    


    <!-- http://purl.obolibrary.org/obo/GAZ_00005432 -->

    <owl:Class rdf:about="http://purl.obolibrary.org/obo/GAZ_00005432"/>
    


    <!-- http://purl.obolibrary.org/obo/GAZ_00005433 -->

    <owl:Class rdf:about="http://purl.obolibrary.org/obo/GAZ_00005433">
        <rdfs:subClassOf rdf:resource="http://purl.obolibrary.org/obo/GAZ_00005432"/>
    </owl:Class>
    


    <!-- http://purl.obolibrary.org/obo/GAZ_00008593 -->

    <owl:Class rdf:about="http://purl.obolibrary.org/obo/GAZ_00008593">
        <rdfs:subClassOf rdf:resource="http://purl.obolibrary.org/obo/GAZ_00005432"/>
    </owl:Class>
    


    <!-- http://purl.obolibrary.org/obo/GAZ_00010058 -->

    <owl:Class rdf:about="http://purl.obolibrary.org/obo/GAZ_00010058">
        <rdfs:subClassOf rdf:resource="http://purl.obolibrary.org/obo/GAZ_00005432"/>
    </owl:Class>
    


    <!-- 
    ///////////////////////////////////////////////////////////////////////////////////////
    //
    // Individuals
    //
    ///////////////////////////////////////////////////////////////////////////////////////
     -->

    


    <!-- http://purl.obolibrary.org/obo/GAZ_00001108 -->

    <owl:NamedIndividual rdf:about="http://purl.obolibrary.org/obo/GAZ_00001108">
        <obo:IAO_0000115>An island nation in the Indian Ocean off the southeastern coast of Africa. The main island, also called Madagascar, is the fourth largest island in the world, and is home to 5% of the world&apos;s plant and animal species, of which more than 80% are endemic to Madagascar. Most notable are the lemur infraorder of primates, the carnivorous fossa, three endemic bird families and six endemic baobab species. Madagascar is divided into six autonomous provinces (faritany mizakatena), and 22 regions. The regions are further subdivided into 116 districts, 1,548 communes, and 16,969 fokontany.</obo:IAO_0000115>
        <oboInOwl:hasOBONamespace>GAZ</oboInOwl:hasOBONamespace>
        <oboInOwl:id>GAZ:00001108</oboInOwl:id>
        <rdfs:label>Madagascar</rdfs:label>
    </owl:NamedIndividual>
    


    <!-- http://purl.obolibrary.org/obo/GAZ_00005421 -->

    <owl:NamedIndividual rdf:about="http://purl.obolibrary.org/obo/GAZ_00005421">
        <obo:RO_0001025 rdf:resource="http://purl.obolibrary.org/obo/GAZ_00001108"/>
    </owl:NamedIndividual>
    


    <!-- http://purl.obolibrary.org/obo/GAZ_00005422 -->

    <owl:NamedIndividual rdf:about="http://purl.obolibrary.org/obo/GAZ_00005422"/>
    


    <!-- http://purl.obolibrary.org/obo/GAZ_00005423 -->

    <owl:NamedIndividual rdf:about="http://purl.obolibrary.org/obo/GAZ_00005423"/>
    


    <!-- http://purl.obolibrary.org/obo/GAZ_00005424 -->

    <owl:NamedIndividual rdf:about="http://purl.obolibrary.org/obo/GAZ_00005424"/>
    


    <!-- http://purl.obolibrary.org/obo/GAZ_00005425 -->

    <owl:NamedIndividual rdf:about="http://purl.obolibrary.org/obo/GAZ_00005425"/>
    


    <!-- http://purl.obolibrary.org/obo/GAZ_00005426 -->

    <owl:NamedIndividual rdf:about="http://purl.obolibrary.org/obo/GAZ_00005426"/>
    


    <!-- http://purl.obolibrary.org/obo/GAZ_00005427 -->

    <owl:NamedIndividual rdf:about="http://purl.obolibrary.org/obo/GAZ_00005427"/>
    


    <!-- http://purl.obolibrary.org/obo/GAZ_00005428 -->

    <owl:NamedIndividual rdf:about="http://purl.obolibrary.org/obo/GAZ_00005428">
        <obo:RO_0001025 rdf:resource="http://purl.obolibrary.org/obo/GAZ_00005423"/>
        <obo:IAO_0000115>A 15,500 hectare protected area consisting principally of primary growth forest in Toamasina Province in eastern Madagascar.</obo:IAO_0000115>
        <oboInOwl:hasOBONamespace>GAZ</oboInOwl:hasOBONamespace>
        <oboInOwl:id>GAZ:00005428</oboInOwl:id>
        <rdfs:label>Andasibe-Mantadia National Park</rdfs:label>
    </owl:NamedIndividual>
    


    <!-- http://purl.obolibrary.org/obo/GAZ_00005429 -->

    <owl:NamedIndividual rdf:about="http://purl.obolibrary.org/obo/GAZ_00005429">
        <obo:RO_0001025 rdf:resource="http://purl.obolibrary.org/obo/GAZ_00001108"/>
        <oboInOwl:hasOBONamespace>GAZ</oboInOwl:hasOBONamespace>
        <oboInOwl:id>GAZ:00005429</oboInOwl:id>
        <rdfs:label>La Mandraka</rdfs:label>
    </owl:NamedIndividual>
    


    <!-- http://purl.obolibrary.org/obo/GAZ_00005430 -->

    <owl:NamedIndividual rdf:about="http://purl.obolibrary.org/obo/GAZ_00005430">
        <obo:RO_0001025 rdf:resource="http://purl.obolibrary.org/obo/GAZ_00005427"/>
        <obo:IAO_0000115>A mountain.</obo:IAO_0000115>
        <oboInOwl:hasOBONamespace>GAZ</oboInOwl:hasOBONamespace>
        <oboInOwl:id>GAZ:00005430</oboInOwl:id>
        <rdfs:label>Lakera</rdfs:label>
    </owl:NamedIndividual>
    


    <!-- http://purl.obolibrary.org/obo/GAZ_00005432 -->

    <owl:NamedIndividual rdf:about="http://purl.obolibrary.org/obo/GAZ_00005432">
        <obo:RO_0001025 rdf:resource="http://purl.obolibrary.org/obo/GAZ_00001108"/>
    </owl:NamedIndividual>
    


    <!-- http://purl.obolibrary.org/obo/GAZ_00005433 -->

    <owl:NamedIndividual rdf:about="http://purl.obolibrary.org/obo/GAZ_00005433">
        <obo:RO_0001025 rdf:resource="http://purl.obolibrary.org/obo/GAZ_00076509"/>
    </owl:NamedIndividual>
    


    <!-- http://purl.obolibrary.org/obo/GAZ_00008593 -->

    <owl:NamedIndividual rdf:about="http://purl.obolibrary.org/obo/GAZ_00008593">
        <rdf:type rdf:resource="http://purl.obolibrary.org/obo/ENVO_00000856"/>
        <obo:RO_0001025 rdf:resource="http://purl.obolibrary.org/obo/GAZ_00076532"/>
    </owl:NamedIndividual>
    


    <!-- http://purl.obolibrary.org/obo/GAZ_00010058 -->

    <owl:NamedIndividual rdf:about="http://purl.obolibrary.org/obo/GAZ_00010058">
        <obo:RO_0001025 rdf:resource="http://purl.obolibrary.org/obo/GAZ_00076482"/>
    </owl:NamedIndividual>
    


    <!-- http://purl.obolibrary.org/obo/GAZ_00032050 -->

    <owl:NamedIndividual rdf:about="http://purl.obolibrary.org/obo/GAZ_00032050">
        <obo:RO_0001025 rdf:resource="http://purl.obolibrary.org/obo/GAZ_00005422"/>
        <obo:IAO_0000115>A region in Madagascar. The region is situated in central-western Madagascar. It is bordered by Betsiboka, Melaky, Menabe, Vakinankaratra, Itasy and Analamanga.</obo:IAO_0000115>
        <oboInOwl:hasOBONamespace>GAZ</oboInOwl:hasOBONamespace>
        <oboInOwl:id>GAZ:00032050</oboInOwl:id>
        <rdfs:label>Bongolava Region</rdfs:label>
    </owl:NamedIndividual>
    


    <!-- http://purl.obolibrary.org/obo/GAZ_00032051 -->

    <owl:NamedIndividual rdf:about="http://purl.obolibrary.org/obo/GAZ_00032051">
        <obo:RO_0001025 rdf:resource="http://purl.obolibrary.org/obo/GAZ_00005422"/>
        <obo:IAO_0000115>A region in Antananarivo Province of central Madagascar. It borders Analamanga region in northeast, Vakinankaratra in south and Bongolava in northwest. The capital of the region is Miarinarivo.</obo:IAO_0000115>
        <oboInOwl:hasOBONamespace>GAZ</oboInOwl:hasOBONamespace>
        <oboInOwl:id>GAZ:00032051</oboInOwl:id>
        <rdfs:label>Itasy Region</rdfs:label>
    </owl:NamedIndividual>
    


    <!-- http://purl.obolibrary.org/obo/GAZ_00032052 -->

    <owl:NamedIndividual rdf:about="http://purl.obolibrary.org/obo/GAZ_00032052">
        <obo:RO_0001025 rdf:resource="http://purl.obolibrary.org/obo/GAZ_00005422"/>
        <obo:IAO_0000115>A region in Madagascar. The region extends mainly into the North of the capital. It is bordered by Betsiboka (North), Bongolava and Itasy (West), Alaotra Mangoro (East) and Vakinankaratra (South).</obo:IAO_0000115>
        <oboInOwl:hasOBONamespace>GAZ</oboInOwl:hasOBONamespace>
        <oboInOwl:id>GAZ:00032052</oboInOwl:id>
        <rdfs:label>Analamanga Region</rdfs:label>
    </owl:NamedIndividual>
    


    <!-- http://purl.obolibrary.org/obo/GAZ_00032053 -->

    <owl:NamedIndividual rdf:about="http://purl.obolibrary.org/obo/GAZ_00032053">
        <obo:RO_0001025 rdf:resource="http://purl.obolibrary.org/obo/GAZ_00005422"/>
        <obo:IAO_0000115>A region in Madagascar.</obo:IAO_0000115>
        <oboInOwl:hasOBONamespace>GAZ</oboInOwl:hasOBONamespace>
        <oboInOwl:id>GAZ:00032053</oboInOwl:id>
        <rdfs:label>Vakinankaratra Region</rdfs:label>
    </owl:NamedIndividual>
    


    <!-- http://purl.obolibrary.org/obo/GAZ_00032054 -->

    <owl:NamedIndividual rdf:about="http://purl.obolibrary.org/obo/GAZ_00032054">
        <obo:RO_0001025 rdf:resource="http://purl.obolibrary.org/obo/GAZ_00005425"/>
        <obo:IAO_0000115>A region in Madagascar. The region is the most northern part of the island. It borders the regions Sava and Sofia.</obo:IAO_0000115>
        <oboInOwl:hasOBONamespace>GAZ</oboInOwl:hasOBONamespace>
        <oboInOwl:id>GAZ:00032054</oboInOwl:id>
        <rdfs:label>Diana Region</rdfs:label>
    </owl:NamedIndividual>
    


    <!-- http://purl.obolibrary.org/obo/GAZ_00032055 -->

    <owl:NamedIndividual rdf:about="http://purl.obolibrary.org/obo/GAZ_00032055">
        <obo:RO_0001025 rdf:resource="http://purl.obolibrary.org/obo/GAZ_00005425"/>
        <obo:IAO_0000115>A region in Antsiranana Province of Madagascar. Its capital is Sambava. The region is situated at the northern part of the east coast of Madagascar. It is bordered by Diana to the North, Sofia to the West and Analanjirofo to the South.</obo:IAO_0000115>
        <oboInOwl:hasOBONamespace>GAZ</oboInOwl:hasOBONamespace>
        <oboInOwl:id>GAZ:00032055</oboInOwl:id>
        <rdfs:label>Sava Region</rdfs:label>
    </owl:NamedIndividual>
    


    <!-- http://purl.obolibrary.org/obo/GAZ_00032056 -->

    <owl:NamedIndividual rdf:about="http://purl.obolibrary.org/obo/GAZ_00032056">
        <obo:RO_0001025 rdf:resource="http://purl.obolibrary.org/obo/GAZ_00005427"/>
        <obo:IAO_0000115>A region in Fianarantsoa Province of central Madagascar. It borders Vakinankaratra Region in north, Atsinanana in northeast, Vatovavy-Fitovinany in southeast, Haute Matsiatra in south, Atsimo-Andrefana in southwest and Menabe in west.</obo:IAO_0000115>
        <oboInOwl:hasOBONamespace>GAZ</oboInOwl:hasOBONamespace>
        <oboInOwl:id>GAZ:00032056</oboInOwl:id>
        <rdfs:label>Amoron&apos;i Mania Region</rdfs:label>
    </owl:NamedIndividual>
    


    <!-- http://purl.obolibrary.org/obo/GAZ_00032057 -->

    <owl:NamedIndividual rdf:about="http://purl.obolibrary.org/obo/GAZ_00032057">
        <obo:RO_0001025 rdf:resource="http://purl.obolibrary.org/obo/GAZ_00005427"/>
        <obo:IAO_0000115>A region in Madagascar. The region extends along the southern part of the east coast of Madagascar. It is bordered by Vatovavy-Fitovinany and Haute Matsiatra (North), Ihorombe (West) and Anosy (South).</obo:IAO_0000115>
        <oboInOwl:hasOBONamespace>GAZ</oboInOwl:hasOBONamespace>
        <oboInOwl:id>GAZ:00032057</oboInOwl:id>
        <rdfs:label>Atsimo-Atsinanana Region</rdfs:label>
    </owl:NamedIndividual>
    


    <!-- http://purl.obolibrary.org/obo/GAZ_00032058 -->

    <owl:NamedIndividual rdf:about="http://purl.obolibrary.org/obo/GAZ_00032058">
        <obo:RO_0001025 rdf:resource="http://purl.obolibrary.org/obo/GAZ_00005427"/>
        <obo:IAO_0000115>A region in Fianarantsoa Province of Madagascar. It borders Amoron&apos;i Mania region in north, Vatovavy-Fitovinany in east, Ihorombe in south and Atsimo-Andrefana in west. The capital of the region is Fianarantsoa.</obo:IAO_0000115>
        <oboInOwl:hasOBONamespace>GAZ</oboInOwl:hasOBONamespace>
        <oboInOwl:id>GAZ:00032058</oboInOwl:id>
        <rdfs:label>Haute Matsiatra Region</rdfs:label>
    </owl:NamedIndividual>
    


    <!-- http://purl.obolibrary.org/obo/GAZ_00032059 -->

    <owl:NamedIndividual rdf:about="http://purl.obolibrary.org/obo/GAZ_00032059">
        <obo:RO_0001025 rdf:resource="http://purl.obolibrary.org/obo/GAZ_00005427"/>
        <obo:IAO_0000115>A region in Fianarantsoa Province of Madagascar. It borders Haute Matsiatra region in north, Atsimo-Atsinanana in east, Anosy in south and Atsimo-Andrefana in west. The capital is Ihosy.</obo:IAO_0000115>
        <oboInOwl:hasOBONamespace>GAZ</oboInOwl:hasOBONamespace>
        <oboInOwl:id>GAZ:00032059</oboInOwl:id>
        <rdfs:label>Ihorombe Region</rdfs:label>
    </owl:NamedIndividual>
    


    <!-- http://purl.obolibrary.org/obo/GAZ_00032060 -->

    <owl:NamedIndividual rdf:about="http://purl.obolibrary.org/obo/GAZ_00032060">
        <obo:RO_0001025 rdf:resource="http://purl.obolibrary.org/obo/GAZ_00005427"/>
        <obo:IAO_0000115>A region in Madagascar. The region extends along the southern part of the east coast of Madagascar. It is bordered by Atsinanana (North), Amoron&apos;i Mania and Haute Matsiatra (West) and Atsimo-Atsinanana (South).</obo:IAO_0000115>
        <oboInOwl:hasOBONamespace>GAZ</oboInOwl:hasOBONamespace>
        <oboInOwl:id>GAZ:00032060</oboInOwl:id>
        <rdfs:label>Vatovavy Fitovinany Region</rdfs:label>
    </owl:NamedIndividual>
    


    <!-- http://purl.obolibrary.org/obo/GAZ_00032061 -->

    <owl:NamedIndividual rdf:about="http://purl.obolibrary.org/obo/GAZ_00032061">
        <obo:RO_0001025 rdf:resource="http://purl.obolibrary.org/obo/GAZ_00005426"/>
        <obo:IAO_0000115>A region in Mahajanga Province of Madagascar. It borders Boeny Region in north, Sofia in northeast, Alaotra-Mangoro in east, Analamanga and Bongolava in south and Melaky in west. The capital of the region is Maevatanana.</obo:IAO_0000115>
        <oboInOwl:hasOBONamespace>GAZ</oboInOwl:hasOBONamespace>
        <oboInOwl:id>GAZ:00032061</oboInOwl:id>
        <rdfs:label>Betsiboka Region</rdfs:label>
    </owl:NamedIndividual>
    


    <!-- http://purl.obolibrary.org/obo/GAZ_00032062 -->

    <owl:NamedIndividual rdf:about="http://purl.obolibrary.org/obo/GAZ_00032062">
        <obo:RO_0001025 rdf:resource="http://purl.obolibrary.org/obo/GAZ_00005426"/>
        <obo:IAO_0000115>A region in Mahajanga Province of western Madagascar. It borders Sofia Region in northeast, Betsiboka in south and Melaky in west. The capital of the region is Mahajanga.</obo:IAO_0000115>
        <oboInOwl:hasOBONamespace>GAZ</oboInOwl:hasOBONamespace>
        <oboInOwl:id>GAZ:00032062</oboInOwl:id>
        <rdfs:label>Boeny Region</rdfs:label>
    </owl:NamedIndividual>
    


    <!-- http://purl.obolibrary.org/obo/GAZ_00032063 -->

    <owl:NamedIndividual rdf:about="http://purl.obolibrary.org/obo/GAZ_00032063">
        <obo:RO_0001025 rdf:resource="http://purl.obolibrary.org/obo/GAZ_00005426"/>
        <obo:IAO_0000115>A region in Mahajanga Province of western Madagascar. It borders Boeny Region in northeast, Betsiboka in east, Bongolava in southeast and Menabe in south. The capital of the region is Maintirano.</obo:IAO_0000115>
        <oboInOwl:hasOBONamespace>GAZ</oboInOwl:hasOBONamespace>
        <oboInOwl:id>GAZ:00032063</oboInOwl:id>
        <rdfs:label>Melaky Region</rdfs:label>
    </owl:NamedIndividual>
    


    <!-- http://purl.obolibrary.org/obo/GAZ_00032064 -->

    <owl:NamedIndividual rdf:about="http://purl.obolibrary.org/obo/GAZ_00032064">
        <obo:RO_0001025 rdf:resource="http://purl.obolibrary.org/obo/GAZ_00005426"/>
        <obo:IAO_0000115>A region in northern Madagascar.</obo:IAO_0000115>
        <oboInOwl:hasOBONamespace>GAZ</oboInOwl:hasOBONamespace>
        <oboInOwl:id>GAZ:00032064</oboInOwl:id>
        <rdfs:label>Sofia Region</rdfs:label>
    </owl:NamedIndividual>
    


    <!-- http://purl.obolibrary.org/obo/GAZ_00032065 -->

    <owl:NamedIndividual rdf:about="http://purl.obolibrary.org/obo/GAZ_00032065">
        <obo:RO_0001025 rdf:resource="http://purl.obolibrary.org/obo/GAZ_00005423"/>
        <obo:IAO_0000115>A region in Toamasina Province of eastern Madagascar. It borders Sofia Region in north, Analanjirofo in northeast, Atsinanana in east, Vakinankaratra in southwest, Analamanga in west and Betsiboka in northwest. The capital of the region is Ambatondrazaka.</obo:IAO_0000115>
        <oboInOwl:hasOBONamespace>GAZ</oboInOwl:hasOBONamespace>
        <oboInOwl:id>GAZ:00032065</oboInOwl:id>
        <rdfs:label>Alaotra Mangoro Region</rdfs:label>
    </owl:NamedIndividual>
    


    <!-- http://purl.obolibrary.org/obo/GAZ_00032066 -->

    <owl:NamedIndividual rdf:about="http://purl.obolibrary.org/obo/GAZ_00032066">
        <obo:RO_0001025 rdf:resource="http://purl.obolibrary.org/obo/GAZ_00005423"/>
        <obo:IAO_0000115>A region in Toamasina Province of northeastern Madagascar. It borders Sava Region in north, Sofia in west, Alaotra-Mangoro in southwest and Atsinanana in south.</obo:IAO_0000115>
        <oboInOwl:hasOBONamespace>GAZ</oboInOwl:hasOBONamespace>
        <oboInOwl:id>GAZ:00032066</oboInOwl:id>
        <rdfs:label>Analanjirofo Region</rdfs:label>
    </owl:NamedIndividual>
    


    <!-- http://purl.obolibrary.org/obo/GAZ_00032067 -->

    <owl:NamedIndividual rdf:about="http://purl.obolibrary.org/obo/GAZ_00032067">
        <obo:RO_0001025 rdf:resource="http://purl.obolibrary.org/obo/GAZ_00005423"/>
        <obo:IAO_0000115>A region in Toamasina Province of eastern Madagascar. It borders Analanjirofo region in north, Alaotra-Mangoro in west, Vakinankaratra and Amoron&apos;i Mania in southwest and Vatovavy-Fitovinany in south. The capital of the region is Toamasina.</obo:IAO_0000115>
        <oboInOwl:hasOBONamespace>GAZ</oboInOwl:hasOBONamespace>
        <oboInOwl:id>GAZ:00032067</oboInOwl:id>
        <rdfs:label>Atsinanana Region</rdfs:label>
    </owl:NamedIndividual>
    


    <!-- http://purl.obolibrary.org/obo/GAZ_00032068 -->

    <owl:NamedIndividual rdf:about="http://purl.obolibrary.org/obo/GAZ_00032068">
        <obo:RO_0001025 rdf:resource="http://purl.obolibrary.org/obo/GAZ_00005424"/>
        <obo:IAO_0000115>A region in Madagascar. Androy is the most southern region of Madagascar. It is bordered by Atsimo-Andrefana (West) and Anosy (East).</obo:IAO_0000115>
        <oboInOwl:hasOBONamespace>GAZ</oboInOwl:hasOBONamespace>
        <oboInOwl:id>GAZ:00032068</oboInOwl:id>
        <rdfs:label>Androy Region</rdfs:label>
    </owl:NamedIndividual>
    


    <!-- http://purl.obolibrary.org/obo/GAZ_00032069 -->

    <owl:NamedIndividual rdf:about="http://purl.obolibrary.org/obo/GAZ_00032069">
        <obo:RO_0001025 rdf:resource="http://purl.obolibrary.org/obo/GAZ_00005424"/>
        <obo:IAO_0000115>A region in Toliara Province of Madagascar. It borders Androy region in west, Atsimo-Andrefana in north-west, Ihorombe in north and Atsimo-Atsinanana in north-east. The capital is Tolanaro.</obo:IAO_0000115>
        <oboInOwl:hasOBONamespace>GAZ</oboInOwl:hasOBONamespace>
        <oboInOwl:id>GAZ:00032069</oboInOwl:id>
        <rdfs:label>Anosy Region</rdfs:label>
    </owl:NamedIndividual>
    


    <!-- http://purl.obolibrary.org/obo/GAZ_00032070 -->

    <owl:NamedIndividual rdf:about="http://purl.obolibrary.org/obo/GAZ_00032070">
        <obo:RO_0001025 rdf:resource="http://purl.obolibrary.org/obo/GAZ_00005424"/>
        <obo:IAO_0000115>A region in Toliara Province of Madagascar. It borders Menabe in north, Amoron&apos;i Mania and Haute Matsiatra in northeast, Ihorombe and Anosy in east and Androy in southeast. The capital is Toliara.</obo:IAO_0000115>
        <oboInOwl:hasOBONamespace>GAZ</oboInOwl:hasOBONamespace>
        <oboInOwl:id>GAZ:00032070</oboInOwl:id>
        <rdfs:label>Atsimo-Andrefana Region</rdfs:label>
    </owl:NamedIndividual>
    


    <!-- http://purl.obolibrary.org/obo/GAZ_00032071 -->

    <owl:NamedIndividual rdf:about="http://purl.obolibrary.org/obo/GAZ_00032071">
        <obo:RO_0001025 rdf:resource="http://purl.obolibrary.org/obo/GAZ_00005424"/>
        <obo:IAO_0000115>A region in Western Madagascar.</obo:IAO_0000115>
        <oboInOwl:hasOBONamespace>GAZ</oboInOwl:hasOBONamespace>
        <oboInOwl:id>GAZ:00032071</oboInOwl:id>
        <rdfs:label>Menabe Region</rdfs:label>
    </owl:NamedIndividual>
    


    <!-- http://purl.obolibrary.org/obo/GAZ_00039953 -->

    <owl:NamedIndividual rdf:about="http://purl.obolibrary.org/obo/GAZ_00039953">
        <rdf:type rdf:resource="http://purl.obolibrary.org/obo/ENVO_00000222"/>
        <obo:RO_0001025 rdf:resource="http://purl.obolibrary.org/obo/GAZ_00076433"/>
        <obo:IAO_0000115>A volcanic island with an area of about 300 km2, and reaches its highest peak at Mont Lokone at 450 m. It is located about eight km off the north-west coast of Madagascar. The island contains very recent basaltic lava flows from well-preserved cinder cones. Many large crater lakes are found in the central part of the island. Nosy-Be volcanics, which are dominantly of low-silica foiditic compositions, overlie Mesozoic limestones and other sedimentary rocks.</obo:IAO_0000115>
        <oboInOwl:hasOBONamespace>GAZ</oboInOwl:hasOBONamespace>
        <oboInOwl:id>GAZ:00039953</oboInOwl:id>
        <rdfs:label>Nosy Bey</rdfs:label>
    </owl:NamedIndividual>
    


    <!-- http://purl.obolibrary.org/obo/GAZ_00039954 -->

    <owl:NamedIndividual rdf:about="http://purl.obolibrary.org/obo/GAZ_00039954">
        <obo:RO_0001025 rdf:resource="http://purl.obolibrary.org/obo/GAZ_00039953"/>
        <oboInOwl:hasOBONamespace>GAZ</oboInOwl:hasOBONamespace>
        <oboInOwl:id>GAZ:00039954</oboInOwl:id>
        <rdfs:label>Commune of Nosy Be</rdfs:label>
    </owl:NamedIndividual>
    


    <!-- http://purl.obolibrary.org/obo/GAZ_00039955 -->

    <owl:NamedIndividual rdf:about="http://purl.obolibrary.org/obo/GAZ_00039955">
        <obo:RO_0001025 rdf:resource="http://purl.obolibrary.org/obo/GAZ_00032054"/>
        <obo:IAO_0000115>A small island near Nosy Be.</obo:IAO_0000115>
        <oboInOwl:hasOBONamespace>GAZ</oboInOwl:hasOBONamespace>
        <oboInOwl:id>GAZ:00039955</oboInOwl:id>
        <rdfs:label>Nosy Sakatia</rdfs:label>
    </owl:NamedIndividual>
    


    <!-- http://purl.obolibrary.org/obo/GAZ_00039956 -->

    <owl:NamedIndividual rdf:about="http://purl.obolibrary.org/obo/GAZ_00039956">
        <obo:RO_0001025 rdf:resource="http://purl.obolibrary.org/obo/GAZ_00032054"/>
        <obo:IAO_0000115>A small island near Nosy Be.</obo:IAO_0000115>
        <oboInOwl:hasOBONamespace>GAZ</oboInOwl:hasOBONamespace>
        <oboInOwl:id>GAZ:00039956</oboInOwl:id>
        <rdfs:label>Nosy Tanikely</rdfs:label>
    </owl:NamedIndividual>
    


    <!-- http://purl.obolibrary.org/obo/GAZ_00039957 -->

    <owl:NamedIndividual rdf:about="http://purl.obolibrary.org/obo/GAZ_00039957">
        <obo:RO_0001025 rdf:resource="http://purl.obolibrary.org/obo/GAZ_00032054"/>
        <obo:IAO_0000115>A small island near Nosy Be.</obo:IAO_0000115>
        <oboInOwl:hasOBONamespace>GAZ</oboInOwl:hasOBONamespace>
        <oboInOwl:id>GAZ:00039957</oboInOwl:id>
        <rdfs:label>Nosy Mitsio</rdfs:label>
    </owl:NamedIndividual>
    


    <!-- http://purl.obolibrary.org/obo/GAZ_00039958 -->

    <owl:NamedIndividual rdf:about="http://purl.obolibrary.org/obo/GAZ_00039958">
        <obo:RO_0001025 rdf:resource="http://purl.obolibrary.org/obo/GAZ_00032054"/>
        <obo:IAO_0000115>A small island near Nosy Be.</obo:IAO_0000115>
        <oboInOwl:hasOBONamespace>GAZ</oboInOwl:hasOBONamespace>
        <oboInOwl:id>GAZ:00039958</oboInOwl:id>
        <rdfs:label>Nosy Komba</rdfs:label>
    </owl:NamedIndividual>
    


    <!-- http://purl.obolibrary.org/obo/GAZ_00039959 -->

    <owl:NamedIndividual rdf:about="http://purl.obolibrary.org/obo/GAZ_00039959">
        <obo:RO_0001025 rdf:resource="http://purl.obolibrary.org/obo/GAZ_00032066"/>
        <obo:IAO_0000115>An island off the east coast of Madagascar.</obo:IAO_0000115>
        <oboInOwl:hasOBONamespace>GAZ</oboInOwl:hasOBONamespace>
        <oboInOwl:id>GAZ:00039959</oboInOwl:id>
        <rdfs:label>Nosy Boraha</rdfs:label>
    </owl:NamedIndividual>
    


    <!-- http://purl.obolibrary.org/obo/GAZ_00051976 -->

    <owl:NamedIndividual rdf:about="http://purl.obolibrary.org/obo/GAZ_00051976">
        <obo:RO_0001025 rdf:resource="http://purl.obolibrary.org/obo/GAZ_00039953"/>
        <obo:IAO_0000115>An island off the NW coast of Madagascar that contains very recent basaltic lava flows from well-preserved cinder cones. Many large crater lakes are found in the central part of the island. Nosy-Be volcanics, which are dominantly of low-silica foiditic compositions, overlie Mesozoic limestones and other sedimentary rocks. Two periods of activity occurred at Nosy-Be. Initial eruptions of fluid lava flows from the western side of the massif were followed by the construction of numerous strombolian cinder cones on the western plain. Little is known about the age of the volcanic field, and the only K-Ar dates are Tertiary in age, but the Nosy-Be volcanics were mapped as Recent (Besairie, 1973).</obo:IAO_0000115>
        <oboInOwl:hasOBONamespace>GAZ</oboInOwl:hasOBONamespace>
        <oboInOwl:id>GAZ:00051976</oboInOwl:id>
        <rdfs:label>Nosy-Be Volcano</rdfs:label>
    </owl:NamedIndividual>
    


    <!-- http://purl.obolibrary.org/obo/GAZ_00053742 -->

    <owl:NamedIndividual rdf:about="http://purl.obolibrary.org/obo/GAZ_00053742">
        <obo:RO_0001025 rdf:resource="http://purl.obolibrary.org/obo/GAZ_00005425"/>
        <obo:IAO_0000115>A volcanic field at the northern tip of Madagascar consists of Miocene volcanics capped by very recent cones. The earliest volcanism produced a large basaltic massif and minor pyroclastic flows. Tertiary to Quaternary volcanic rocks span a wide geochemical spectrum, including basaltic, andesitic, rhyolitic, trachytic, phonolitic, and foiditic compositions.</obo:IAO_0000115>
        <oboInOwl:hasOBONamespace>GAZ</oboInOwl:hasOBONamespace>
        <oboInOwl:id>GAZ:00053742</oboInOwl:id>
        <rdfs:label>Ambre-Bobaomby Volcanic Field</rdfs:label>
    </owl:NamedIndividual>
    


    <!-- http://purl.obolibrary.org/obo/GAZ_00053743 -->

    <owl:NamedIndividual rdf:about="http://purl.obolibrary.org/obo/GAZ_00053743">
        <obo:RO_0001025 rdf:resource="http://purl.obolibrary.org/obo/GAZ_00001108"/>
        <obo:IAO_0000115>A volcanic field, covering portions of the Tsaratanana and Ambondrona massifs in northern Madagascar, was active until the very recent Quaternary. An initial dominantly silicic phase included pyroclastic-flow formation and was accompanied by the emission of minor basaltic lava flows. An earlier now-eroded basaltic phase was followed by the most recent activity, which produced a series of perfectly preserved cinder cones and lava flows that traveled down current valley floors in the Bealanana region.</obo:IAO_0000115>
        <oboInOwl:hasOBONamespace>GAZ</oboInOwl:hasOBONamespace>
        <oboInOwl:id>GAZ:00053743</oboInOwl:id>
        <rdfs:label>Ankaizina Volcanic Field</rdfs:label>
    </owl:NamedIndividual>
    


    <!-- http://purl.obolibrary.org/obo/GAZ_00053744 -->

    <owl:NamedIndividual rdf:about="http://purl.obolibrary.org/obo/GAZ_00053744">
        <obo:RO_0001025 rdf:resource="http://purl.obolibrary.org/obo/GAZ_00001108"/>
        <obo:IAO_0000115>A volcanic field in central Madagascar that contains a diverse assemblage of volcanic landforms, including scoria cones, lava domes, and maars. Activity began in the Pliocene and has continued into the Holocene. Early eruptions produced trachytic lava domes and basanitic lava flows. Later activity produced trachytic lava flows and recent vulcanian eruptions. A trachytic maar was formed near Saovinandriana at the beginning of the Holocene, and several other crater lakes are present. Mild seismicity and thermal activity in the form of hot springs continues at Itasy.</obo:IAO_0000115>
        <oboInOwl:hasOBONamespace>GAZ</oboInOwl:hasOBONamespace>
        <oboInOwl:id>GAZ:00053744</oboInOwl:id>
        <rdfs:label>Itasy Volcanic Field</rdfs:label>
    </owl:NamedIndividual>
    


    <!-- http://purl.obolibrary.org/obo/GAZ_00053745 -->

    <owl:NamedIndividual rdf:about="http://purl.obolibrary.org/obo/GAZ_00053745">
        <obo:RO_0001025 rdf:resource="http://purl.obolibrary.org/obo/GAZ_00001108"/>
        <obo:IAO_0000115>A volcanic field that covers a 100 km-long area in central Madagascar between Avivonimamo and Antsirabe. Activity at the Ankaratra volcanic massif took place from the Miocene until the very recent Quaternary (Besairie, 1973). Trachytic lava domes were erupted during the initial stage and massive fissure eruptions created a series of tectonic lakes. The latest activity occurred in the southern part of the massif and produced well-preserved strombolian basanitic cinder cones. Vulcanian eruptions formed several lake-filled craters. Hot springs occur at Ranomafana.</obo:IAO_0000115>
        <oboInOwl:hasOBONamespace>GAZ</oboInOwl:hasOBONamespace>
        <oboInOwl:id>GAZ:00053745</oboInOwl:id>
        <rdfs:label>Ankaratra Volcanic Field</rdfs:label>
    </owl:NamedIndividual>
    


    <!-- http://purl.obolibrary.org/obo/GAZ_00058830 -->

    <owl:NamedIndividual rdf:about="http://purl.obolibrary.org/obo/GAZ_00058830">
        <obo:RO_0001025 rdf:resource="http://purl.obolibrary.org/obo/GAZ_00005423"/>
        <obo:IAO_0000115>A lake located in Toamasina Province, in the northern central plateau. The Ambato River provides the Lake with water and also drains it. A Ramsar Site.</obo:IAO_0000115>
        <oboInOwl:hasOBONamespace>GAZ</oboInOwl:hasOBONamespace>
        <oboInOwl:id>GAZ:00058830</oboInOwl:id>
        <rdfs:label>Lake Alaotra</rdfs:label>
    </owl:NamedIndividual>
    


    <!-- http://purl.obolibrary.org/obo/GAZ_00058831 -->

    <owl:NamedIndividual rdf:about="http://purl.obolibrary.org/obo/GAZ_00058831">
        <obo:RO_0001025 rdf:resource="http://purl.obolibrary.org/obo/GAZ_00005424"/>
        <obo:IAO_0000115>An endorheic saline lake in semi-arid southwestern part of Madagascar.</obo:IAO_0000115>
        <oboInOwl:hasOBONamespace>GAZ</oboInOwl:hasOBONamespace>
        <oboInOwl:id>GAZ:00058831</oboInOwl:id>
        <rdfs:label>Lake Ihotry</rdfs:label>
    </owl:NamedIndividual>
    


    <!-- http://purl.obolibrary.org/obo/GAZ_00058832 -->

    <owl:NamedIndividual rdf:about="http://purl.obolibrary.org/obo/GAZ_00058832">
        <obo:RO_0001025 rdf:resource="http://purl.obolibrary.org/obo/GAZ_00005426"/>
        <obo:IAO_0000115>A lake in northwestern part of Madagascar, in the Mahajanga Province.</obo:IAO_0000115>
        <oboInOwl:hasOBONamespace>GAZ</oboInOwl:hasOBONamespace>
        <oboInOwl:id>GAZ:00058832</oboInOwl:id>
        <rdfs:label>Lake Kinkony</rdfs:label>
    </owl:NamedIndividual>
    


    <!-- http://purl.obolibrary.org/obo/GAZ_00058833 -->

    <owl:NamedIndividual rdf:about="http://purl.obolibrary.org/obo/GAZ_00058833">
        <obo:RO_0001025 rdf:resource="http://purl.obolibrary.org/obo/GAZ_00005422"/>
        <obo:IAO_0000115>A crater lake in Madagascar.</obo:IAO_0000115>
        <oboInOwl:hasOBONamespace>GAZ</oboInOwl:hasOBONamespace>
        <oboInOwl:id>GAZ:00058833</oboInOwl:id>
        <rdfs:label>Lake Tritriva</rdfs:label>
    </owl:NamedIndividual>
    


    <!-- http://purl.obolibrary.org/obo/GAZ_00058834 -->

    <owl:NamedIndividual rdf:about="http://purl.obolibrary.org/obo/GAZ_00058834">
        <obo:RO_0001025 rdf:resource="http://purl.obolibrary.org/obo/GAZ_00005424"/>
        <obo:IAO_0000115>A saline lake in the Toliara Province, southwestern part of Madagascar. A Ramsar Site.</obo:IAO_0000115>
        <oboInOwl:hasOBONamespace>GAZ</oboInOwl:hasOBONamespace>
        <oboInOwl:id>GAZ:00058834</oboInOwl:id>
        <rdfs:label>Lake Tsimanampetsotsa</rdfs:label>
    </owl:NamedIndividual>
    


    <!-- http://purl.obolibrary.org/obo/GAZ_00076432 -->

    <owl:NamedIndividual rdf:about="http://purl.obolibrary.org/obo/GAZ_00076432">
        <rdf:type rdf:resource="http://purl.obolibrary.org/obo/ENVO_00000004"/>
        <obo:RO_0001025 rdf:resource="http://purl.obolibrary.org/obo/GAZ_00032054"/>
        <obo:IAO_0000115>A district in the Diana Region of Madagascar.</obo:IAO_0000115>
        <oboInOwl:hasOBONamespace>GAZ</oboInOwl:hasOBONamespace>
        <oboInOwl:id>GAZ:00076432</oboInOwl:id>
        <rdfs:label>Antsiranana I District</rdfs:label>
    </owl:NamedIndividual>
    


    <!-- http://purl.obolibrary.org/obo/GAZ_00076433 -->

    <owl:NamedIndividual rdf:about="http://purl.obolibrary.org/obo/GAZ_00076433">
        <rdf:type rdf:resource="http://purl.obolibrary.org/obo/ENVO_00000004"/>
        <obo:RO_0001025 rdf:resource="http://purl.obolibrary.org/obo/GAZ_00032054"/>
        <obo:IAO_0000115>A district in the Diana Region of Madagascar.</obo:IAO_0000115>
        <oboInOwl:hasOBONamespace>GAZ</oboInOwl:hasOBONamespace>
        <oboInOwl:id>GAZ:00076433</oboInOwl:id>
        <rdfs:label>Nosy Be District</rdfs:label>
    </owl:NamedIndividual>
    


    <!-- http://purl.obolibrary.org/obo/GAZ_00076434 -->

    <owl:NamedIndividual rdf:about="http://purl.obolibrary.org/obo/GAZ_00076434">
        <rdf:type rdf:resource="http://purl.obolibrary.org/obo/ENVO_00000004"/>
        <obo:RO_0001025 rdf:resource="http://purl.obolibrary.org/obo/GAZ_00032054"/>
        <obo:IAO_0000115>A district in the Diana Region of Madagascar.</obo:IAO_0000115>
        <oboInOwl:hasOBONamespace>GAZ</oboInOwl:hasOBONamespace>
        <oboInOwl:id>GAZ:00076434</oboInOwl:id>
        <rdfs:label>Antsiranana II District</rdfs:label>
    </owl:NamedIndividual>
    


    <!-- http://purl.obolibrary.org/obo/GAZ_00076435 -->

    <owl:NamedIndividual rdf:about="http://purl.obolibrary.org/obo/GAZ_00076435">
        <rdf:type rdf:resource="http://purl.obolibrary.org/obo/ENVO_00000004"/>
        <obo:RO_0001025 rdf:resource="http://purl.obolibrary.org/obo/GAZ_00032054"/>
        <obo:IAO_0000115>A district in the Diana Region of Madagascar.</obo:IAO_0000115>
        <oboInOwl:hasOBONamespace>GAZ</oboInOwl:hasOBONamespace>
        <oboInOwl:id>GAZ:00076435</oboInOwl:id>
        <rdfs:label>Ambanja District</rdfs:label>
    </owl:NamedIndividual>
    


    <!-- http://purl.obolibrary.org/obo/GAZ_00076436 -->

    <owl:NamedIndividual rdf:about="http://purl.obolibrary.org/obo/GAZ_00076436">
        <rdf:type rdf:resource="http://purl.obolibrary.org/obo/ENVO_00000004"/>
        <obo:RO_0001025 rdf:resource="http://purl.obolibrary.org/obo/GAZ_00032054"/>
        <obo:IAO_0000115>A district in the Diana Region of Madagascar.</obo:IAO_0000115>
        <oboInOwl:hasOBONamespace>GAZ</oboInOwl:hasOBONamespace>
        <oboInOwl:id>GAZ:00076436</oboInOwl:id>
        <rdfs:label>Ambilobe District</rdfs:label>
    </owl:NamedIndividual>
    


    <!-- http://purl.obolibrary.org/obo/GAZ_00076437 -->

    <owl:NamedIndividual rdf:about="http://purl.obolibrary.org/obo/GAZ_00076437">
        <rdf:type rdf:resource="http://purl.obolibrary.org/obo/ENVO_00000004"/>
        <obo:RO_0001025 rdf:resource="http://purl.obolibrary.org/obo/GAZ_00032055"/>
        <obo:IAO_0000115>A district in the Sava Region of Antsiranana Province, and borders the districts of Sambava in north, Andapa in north-west and Maroantsetra in west.</obo:IAO_0000115>
        <oboInOwl:hasOBONamespace>GAZ</oboInOwl:hasOBONamespace>
        <oboInOwl:id>GAZ:00076437</oboInOwl:id>
        <rdfs:label>Antalaha District</rdfs:label>
    </owl:NamedIndividual>
    


    <!-- http://purl.obolibrary.org/obo/GAZ_00076438 -->

    <owl:NamedIndividual rdf:about="http://purl.obolibrary.org/obo/GAZ_00076438">
        <rdf:type rdf:resource="http://purl.obolibrary.org/obo/ENVO_00000004"/>
        <obo:RO_0001025 rdf:resource="http://purl.obolibrary.org/obo/GAZ_00032055"/>
        <obo:IAO_0000115>A district in northern Madagascar. It is a part of Sava Region of Antsiranana Province, and borders the districts of Sambava in south, Ambilobe in west and Antsiranana II in north.</obo:IAO_0000115>
        <oboInOwl:hasOBONamespace>GAZ</oboInOwl:hasOBONamespace>
        <oboInOwl:id>GAZ:00076438</oboInOwl:id>
        <rdfs:label>Vohemar District</rdfs:label>
    </owl:NamedIndividual>
    


    <!-- http://purl.obolibrary.org/obo/GAZ_00076439 -->

    <owl:NamedIndividual rdf:about="http://purl.obolibrary.org/obo/GAZ_00076439">
        <rdf:type rdf:resource="http://purl.obolibrary.org/obo/ENVO_00000004"/>
        <obo:RO_0001025 rdf:resource="http://purl.obolibrary.org/obo/GAZ_00032055"/>
        <obo:IAO_0000115>A district in northern Madagascar. It is a part of Sava Region of Antsiranana Province, and borders the districts of Ambilobe and Sambava in north, Antalaha in east, Maroantsetra in south and Befandriana Nord and Bealanana in west.</obo:IAO_0000115>
        <oboInOwl:hasOBONamespace>GAZ</oboInOwl:hasOBONamespace>
        <oboInOwl:id>GAZ:00076439</oboInOwl:id>
        <rdfs:label>Andapa District</rdfs:label>
    </owl:NamedIndividual>
    


    <!-- http://purl.obolibrary.org/obo/GAZ_00076440 -->

    <owl:NamedIndividual rdf:about="http://purl.obolibrary.org/obo/GAZ_00076440">
        <rdf:type rdf:resource="http://purl.obolibrary.org/obo/ENVO_00000004"/>
        <obo:RO_0001025 rdf:resource="http://purl.obolibrary.org/obo/GAZ_00032055"/>
        <obo:IAO_0000115>A district in the Sava Region of Antsiranana Province, and borders the districts of Antalaha in south, Andapa in south-west, Ambilobe in north-west and Vohemar in north.</obo:IAO_0000115>
        <oboInOwl:hasOBONamespace>GAZ</oboInOwl:hasOBONamespace>
        <oboInOwl:id>GAZ:00076440</oboInOwl:id>
        <rdfs:label>Sambava District</rdfs:label>
    </owl:NamedIndividual>
    


    <!-- http://purl.obolibrary.org/obo/GAZ_00076441 -->

    <owl:NamedIndividual rdf:about="http://purl.obolibrary.org/obo/GAZ_00076441">
        <rdf:type rdf:resource="http://purl.obolibrary.org/obo/ENVO_00000004"/>
        <obo:RO_0001025 rdf:resource="http://purl.obolibrary.org/obo/GAZ_00032052"/>
        <obo:IAO_0000115>A district in the Analamanga Region, Madagascar.</obo:IAO_0000115>
        <oboInOwl:hasOBONamespace>GAZ</oboInOwl:hasOBONamespace>
        <oboInOwl:id>GAZ:00076441</oboInOwl:id>
        <rdfs:label>Antananarivo-Atsimondrano District</rdfs:label>
    </owl:NamedIndividual>
    


    <!-- http://purl.obolibrary.org/obo/GAZ_00076442 -->

    <owl:NamedIndividual rdf:about="http://purl.obolibrary.org/obo/GAZ_00076442">
        <rdf:type rdf:resource="http://purl.obolibrary.org/obo/ENVO_00000004"/>
        <obo:RO_0001025 rdf:resource="http://purl.obolibrary.org/obo/GAZ_00032052"/>
        <obo:IAO_0000115>A district in the Analamanga Region, Madagascar.</obo:IAO_0000115>
        <oboInOwl:hasOBONamespace>GAZ</oboInOwl:hasOBONamespace>
        <oboInOwl:id>GAZ:00076442</oboInOwl:id>
        <rdfs:label>Andramasina District</rdfs:label>
    </owl:NamedIndividual>
    


    <!-- http://purl.obolibrary.org/obo/GAZ_00076443 -->

    <owl:NamedIndividual rdf:about="http://purl.obolibrary.org/obo/GAZ_00076443">
        <rdf:type rdf:resource="http://purl.obolibrary.org/obo/ENVO_00000004"/>
        <obo:RO_0001025 rdf:resource="http://purl.obolibrary.org/obo/GAZ_00032052"/>
        <obo:IAO_0000115>A district in the Analamanga Region, Madagascar.</obo:IAO_0000115>
        <oboInOwl:hasOBONamespace>GAZ</oboInOwl:hasOBONamespace>
        <oboInOwl:id>GAZ:00076443</oboInOwl:id>
        <rdfs:label>Manjakandriana District</rdfs:label>
    </owl:NamedIndividual>
    


    <!-- http://purl.obolibrary.org/obo/GAZ_00076444 -->

    <owl:NamedIndividual rdf:about="http://purl.obolibrary.org/obo/GAZ_00076444">
        <rdf:type rdf:resource="http://purl.obolibrary.org/obo/ENVO_00000004"/>
        <obo:RO_0001025 rdf:resource="http://purl.obolibrary.org/obo/GAZ_00032052"/>
        <obo:IAO_0000115>A district in the Analamanga Region, Madagascar.</obo:IAO_0000115>
        <oboInOwl:hasOBONamespace>GAZ</oboInOwl:hasOBONamespace>
        <oboInOwl:id>GAZ:00076444</oboInOwl:id>
        <rdfs:label>Antananarivo-Avaradrano District</rdfs:label>
    </owl:NamedIndividual>
    


    <!-- http://purl.obolibrary.org/obo/GAZ_00076445 -->

    <owl:NamedIndividual rdf:about="http://purl.obolibrary.org/obo/GAZ_00076445">
        <rdf:type rdf:resource="http://purl.obolibrary.org/obo/ENVO_00000004"/>
        <obo:RO_0001025 rdf:resource="http://purl.obolibrary.org/obo/GAZ_00032052"/>
        <obo:IAO_0000115>A district in the Analamanga Region, Madagascar.</obo:IAO_0000115>
        <oboInOwl:hasOBONamespace>GAZ</oboInOwl:hasOBONamespace>
        <oboInOwl:id>GAZ:00076445</oboInOwl:id>
        <rdfs:label>Ankazobe District</rdfs:label>
    </owl:NamedIndividual>
    


    <!-- http://purl.obolibrary.org/obo/GAZ_00076446 -->

    <owl:NamedIndividual rdf:about="http://purl.obolibrary.org/obo/GAZ_00076446">
        <rdf:type rdf:resource="http://purl.obolibrary.org/obo/ENVO_00000004"/>
        <obo:RO_0001025 rdf:resource="http://purl.obolibrary.org/obo/GAZ_00032052"/>
        <obo:IAO_0000115>A district in the Analamanga Region, Madagascar.</obo:IAO_0000115>
        <oboInOwl:hasOBONamespace>GAZ</oboInOwl:hasOBONamespace>
        <oboInOwl:id>GAZ:00076446</oboInOwl:id>
        <rdfs:label>Antananarivo-Renivohitra District</rdfs:label>
    </owl:NamedIndividual>
    


    <!-- http://purl.obolibrary.org/obo/GAZ_00076447 -->

    <owl:NamedIndividual rdf:about="http://purl.obolibrary.org/obo/GAZ_00076447">
        <rdf:type rdf:resource="http://purl.obolibrary.org/obo/ENVO_00000004"/>
        <obo:RO_0001025 rdf:resource="http://purl.obolibrary.org/obo/GAZ_00032052"/>
        <obo:IAO_0000115>A district in the Analamanga Region, Madagascar.</obo:IAO_0000115>
        <oboInOwl:hasOBONamespace>GAZ</oboInOwl:hasOBONamespace>
        <oboInOwl:id>GAZ:00076447</oboInOwl:id>
        <rdfs:label>Ambohidratrimo District</rdfs:label>
    </owl:NamedIndividual>
    


    <!-- http://purl.obolibrary.org/obo/GAZ_00076448 -->

    <owl:NamedIndividual rdf:about="http://purl.obolibrary.org/obo/GAZ_00076448">
        <rdf:type rdf:resource="http://purl.obolibrary.org/obo/ENVO_00000004"/>
        <obo:RO_0001025 rdf:resource="http://purl.obolibrary.org/obo/GAZ_00032052"/>
        <obo:IAO_0000115>A district in the Analamanga Region, Madagascar.</obo:IAO_0000115>
        <oboInOwl:hasOBONamespace>GAZ</oboInOwl:hasOBONamespace>
        <oboInOwl:id>GAZ:00076448</oboInOwl:id>
        <rdfs:label>Anjozorobe District</rdfs:label>
    </owl:NamedIndividual>
    


    <!-- http://purl.obolibrary.org/obo/GAZ_00076449 -->

    <owl:NamedIndividual rdf:about="http://purl.obolibrary.org/obo/GAZ_00076449">
        <rdf:type rdf:resource="http://purl.obolibrary.org/obo/ENVO_00000004"/>
        <obo:RO_0001025 rdf:resource="http://purl.obolibrary.org/obo/GAZ_00032050"/>
        <obo:IAO_0000115>A district in Bongolava Region, Madagascar.</obo:IAO_0000115>
        <oboInOwl:hasOBONamespace>GAZ</oboInOwl:hasOBONamespace>
        <oboInOwl:id>GAZ:00076449</oboInOwl:id>
        <rdfs:label>Tsiroanomandidy District</rdfs:label>
    </owl:NamedIndividual>
    


    <!-- http://purl.obolibrary.org/obo/GAZ_00076450 -->

    <owl:NamedIndividual rdf:about="http://purl.obolibrary.org/obo/GAZ_00076450">
        <rdf:type rdf:resource="http://purl.obolibrary.org/obo/ENVO_00000004"/>
        <obo:RO_0001025 rdf:resource="http://purl.obolibrary.org/obo/GAZ_00032050"/>
        <obo:IAO_0000115>A district in Bongolava Region, Madagascar.</obo:IAO_0000115>
        <oboInOwl:hasOBONamespace>GAZ</oboInOwl:hasOBONamespace>
        <oboInOwl:id>GAZ:00076450</oboInOwl:id>
        <rdfs:label>Fenoarivobe District</rdfs:label>
    </owl:NamedIndividual>
    


    <!-- http://purl.obolibrary.org/obo/GAZ_00076451 -->

    <owl:NamedIndividual rdf:about="http://purl.obolibrary.org/obo/GAZ_00076451">
        <rdf:type rdf:resource="http://purl.obolibrary.org/obo/ENVO_00000004"/>
        <obo:RO_0001025 rdf:resource="http://purl.obolibrary.org/obo/GAZ_00032051"/>
        <obo:IAO_0000115>A district in Itasy Region, Madagascar.</obo:IAO_0000115>
        <oboInOwl:hasOBONamespace>GAZ</oboInOwl:hasOBONamespace>
        <oboInOwl:id>GAZ:00076451</oboInOwl:id>
        <rdfs:label>Miarinarivo District</rdfs:label>
    </owl:NamedIndividual>
    


    <!-- http://purl.obolibrary.org/obo/GAZ_00076452 -->

    <owl:NamedIndividual rdf:about="http://purl.obolibrary.org/obo/GAZ_00076452">
        <rdf:type rdf:resource="http://purl.obolibrary.org/obo/ENVO_00000004"/>
        <obo:RO_0001025 rdf:resource="http://purl.obolibrary.org/obo/GAZ_00032051"/>
        <obo:IAO_0000115>A district in Itasy Region, Madagascar.</obo:IAO_0000115>
        <oboInOwl:hasOBONamespace>GAZ</oboInOwl:hasOBONamespace>
        <oboInOwl:id>GAZ:00076452</oboInOwl:id>
        <rdfs:label>Arivonimamo District</rdfs:label>
    </owl:NamedIndividual>
    


    <!-- http://purl.obolibrary.org/obo/GAZ_00076453 -->

    <owl:NamedIndividual rdf:about="http://purl.obolibrary.org/obo/GAZ_00076453">
        <rdf:type rdf:resource="http://purl.obolibrary.org/obo/ENVO_00000004"/>
        <obo:RO_0001025 rdf:resource="http://purl.obolibrary.org/obo/GAZ_00032051"/>
        <obo:IAO_0000115>A district in Itasy Region, Madagascar.</obo:IAO_0000115>
        <oboInOwl:hasOBONamespace>GAZ</oboInOwl:hasOBONamespace>
        <oboInOwl:id>GAZ:00076453</oboInOwl:id>
        <rdfs:label>Soavinandriana District</rdfs:label>
    </owl:NamedIndividual>
    


    <!-- http://purl.obolibrary.org/obo/GAZ_00076454 -->

    <owl:NamedIndividual rdf:about="http://purl.obolibrary.org/obo/GAZ_00076454">
        <rdf:type rdf:resource="http://purl.obolibrary.org/obo/ENVO_00000004"/>
        <obo:RO_0001025 rdf:resource="http://purl.obolibrary.org/obo/GAZ_00032053"/>
        <obo:IAO_0000115>A district in Vakinankaratra Region, Madagascar.</obo:IAO_0000115>
        <oboInOwl:hasOBONamespace>GAZ</oboInOwl:hasOBONamespace>
        <oboInOwl:id>GAZ:00076454</oboInOwl:id>
        <rdfs:label>Betafo District</rdfs:label>
    </owl:NamedIndividual>
    


    <!-- http://purl.obolibrary.org/obo/GAZ_00076455 -->

    <owl:NamedIndividual rdf:about="http://purl.obolibrary.org/obo/GAZ_00076455">
        <rdf:type rdf:resource="http://purl.obolibrary.org/obo/ENVO_00000004"/>
        <obo:RO_0001025 rdf:resource="http://purl.obolibrary.org/obo/GAZ_00032053"/>
        <obo:IAO_0000115>A district in Vakinankaratra Region, Madagascar.</obo:IAO_0000115>
        <oboInOwl:hasOBONamespace>GAZ</oboInOwl:hasOBONamespace>
        <oboInOwl:id>GAZ:00076455</oboInOwl:id>
        <rdfs:label>Faratsiho District</rdfs:label>
    </owl:NamedIndividual>
    


    <!-- http://purl.obolibrary.org/obo/GAZ_00076456 -->

    <owl:NamedIndividual rdf:about="http://purl.obolibrary.org/obo/GAZ_00076456">
        <rdf:type rdf:resource="http://purl.obolibrary.org/obo/ENVO_00000004"/>
        <obo:RO_0001025 rdf:resource="http://purl.obolibrary.org/obo/GAZ_00032053"/>
        <obo:IAO_0000115>A district in Vakinankaratra Region, Madagascar.</obo:IAO_0000115>
        <oboInOwl:hasOBONamespace>GAZ</oboInOwl:hasOBONamespace>
        <oboInOwl:id>GAZ:00076456</oboInOwl:id>
        <rdfs:label>Antsirabe I District</rdfs:label>
    </owl:NamedIndividual>
    


    <!-- http://purl.obolibrary.org/obo/GAZ_00076457 -->

    <owl:NamedIndividual rdf:about="http://purl.obolibrary.org/obo/GAZ_00076457">
        <rdf:type rdf:resource="http://purl.obolibrary.org/obo/ENVO_00000004"/>
        <obo:RO_0001025 rdf:resource="http://purl.obolibrary.org/obo/GAZ_00032053"/>
        <obo:IAO_0000115>A district in Vakinankaratra Region, Madagascar.</obo:IAO_0000115>
        <oboInOwl:hasOBONamespace>GAZ</oboInOwl:hasOBONamespace>
        <oboInOwl:id>GAZ:00076457</oboInOwl:id>
        <rdfs:label>Ambatolampy District</rdfs:label>
    </owl:NamedIndividual>
    


    <!-- http://purl.obolibrary.org/obo/GAZ_00076458 -->

    <owl:NamedIndividual rdf:about="http://purl.obolibrary.org/obo/GAZ_00076458">
        <rdf:type rdf:resource="http://purl.obolibrary.org/obo/ENVO_00000004"/>
        <obo:RO_0001025 rdf:resource="http://purl.obolibrary.org/obo/GAZ_00032053"/>
        <obo:IAO_0000115>A district in Vakinankaratra Region, Madagascar.</obo:IAO_0000115>
        <oboInOwl:hasOBONamespace>GAZ</oboInOwl:hasOBONamespace>
        <oboInOwl:id>GAZ:00076458</oboInOwl:id>
        <rdfs:label>Antanifotsy District</rdfs:label>
    </owl:NamedIndividual>
    


    <!-- http://purl.obolibrary.org/obo/GAZ_00076459 -->

    <owl:NamedIndividual rdf:about="http://purl.obolibrary.org/obo/GAZ_00076459">
        <rdf:type rdf:resource="http://purl.obolibrary.org/obo/ENVO_00000004"/>
        <obo:RO_0001025 rdf:resource="http://purl.obolibrary.org/obo/GAZ_00032053"/>
        <obo:IAO_0000115>A district in Vakinankaratra Region, Madagascar.</obo:IAO_0000115>
        <oboInOwl:hasOBONamespace>GAZ</oboInOwl:hasOBONamespace>
        <oboInOwl:id>GAZ:00076459</oboInOwl:id>
        <rdfs:label>Antsirabe II District</rdfs:label>
    </owl:NamedIndividual>
    


    <!-- http://purl.obolibrary.org/obo/GAZ_00076460 -->

    <owl:NamedIndividual rdf:about="http://purl.obolibrary.org/obo/GAZ_00076460">
        <obo:RO_0001025 rdf:resource="http://purl.obolibrary.org/obo/GAZ_00005427"/>
        <oboInOwl:hasOBONamespace>GAZ</oboInOwl:hasOBONamespace>
        <oboInOwl:id>GAZ:00076460</oboInOwl:id>
        <rdfs:label>Midongy Du Sud National Park</rdfs:label>
    </owl:NamedIndividual>
    


    <!-- http://purl.obolibrary.org/obo/GAZ_00076461 -->

    <owl:NamedIndividual rdf:about="http://purl.obolibrary.org/obo/GAZ_00076461">
        <obo:RO_0001025 rdf:resource="http://purl.obolibrary.org/obo/GAZ_00005427"/>
        <obo:IAO_0000115>A national park located in the southeastern part of Madagascar. Established 1991.</obo:IAO_0000115>
        <oboInOwl:hasOBONamespace>GAZ</oboInOwl:hasOBONamespace>
        <oboInOwl:id>GAZ:00076461</oboInOwl:id>
        <rdfs:label>Ranomafana National Park</rdfs:label>
    </owl:NamedIndividual>
    


    <!-- http://purl.obolibrary.org/obo/GAZ_00076463 -->

    <owl:NamedIndividual rdf:about="http://purl.obolibrary.org/obo/GAZ_00076463">
        <obo:RO_0001025 rdf:resource="http://purl.obolibrary.org/obo/GAZ_00005427"/>
        <obo:IAO_0000115>A national park in the Fianarantsoa Province of Madagascar.</obo:IAO_0000115>
        <oboInOwl:hasOBONamespace>GAZ</oboInOwl:hasOBONamespace>
        <oboInOwl:id>GAZ:00076463</oboInOwl:id>
        <rdfs:label>Isalo National Park</rdfs:label>
    </owl:NamedIndividual>
    


    <!-- http://purl.obolibrary.org/obo/GAZ_00076464 -->

    <owl:NamedIndividual rdf:about="http://purl.obolibrary.org/obo/GAZ_00076464">
        <rdf:type rdf:resource="http://purl.obolibrary.org/obo/ENVO_00000004"/>
        <obo:RO_0001025 rdf:resource="http://purl.obolibrary.org/obo/GAZ_00032056"/>
        <obo:IAO_0000115>A district in Amoron&apos;i Mania Region, Madagascar.</obo:IAO_0000115>
        <oboInOwl:hasOBONamespace>GAZ</oboInOwl:hasOBONamespace>
        <oboInOwl:id>GAZ:00076464</oboInOwl:id>
        <rdfs:label>Ambatofinandrahana District</rdfs:label>
    </owl:NamedIndividual>
    


    <!-- http://purl.obolibrary.org/obo/GAZ_00076465 -->

    <owl:NamedIndividual rdf:about="http://purl.obolibrary.org/obo/GAZ_00076465">
        <rdf:type rdf:resource="http://purl.obolibrary.org/obo/ENVO_00000004"/>
        <obo:RO_0001025 rdf:resource="http://purl.obolibrary.org/obo/GAZ_00032056"/>
        <obo:IAO_0000115>A district in Amoron&apos;i Mania Region, Madagascar.</obo:IAO_0000115>
        <oboInOwl:hasOBONamespace>GAZ</oboInOwl:hasOBONamespace>
        <oboInOwl:id>GAZ:00076465</oboInOwl:id>
        <rdfs:label>Fandriana District</rdfs:label>
    </owl:NamedIndividual>
    


    <!-- http://purl.obolibrary.org/obo/GAZ_00076466 -->

    <owl:NamedIndividual rdf:about="http://purl.obolibrary.org/obo/GAZ_00076466">
        <rdf:type rdf:resource="http://purl.obolibrary.org/obo/ENVO_00000004"/>
        <obo:RO_0001025 rdf:resource="http://purl.obolibrary.org/obo/GAZ_00032056"/>
        <obo:IAO_0000115>A district in Amoron&apos;i Mania Region, Madagascar.</obo:IAO_0000115>
        <oboInOwl:hasOBONamespace>GAZ</oboInOwl:hasOBONamespace>
        <oboInOwl:id>GAZ:00076466</oboInOwl:id>
        <rdfs:label>Manandriana District</rdfs:label>
    </owl:NamedIndividual>
    


    <!-- http://purl.obolibrary.org/obo/GAZ_00076467 -->

    <owl:NamedIndividual rdf:about="http://purl.obolibrary.org/obo/GAZ_00076467">
        <rdf:type rdf:resource="http://purl.obolibrary.org/obo/ENVO_00000004"/>
        <obo:RO_0001025 rdf:resource="http://purl.obolibrary.org/obo/GAZ_00032056"/>
        <obo:IAO_0000115>A district in Amoron&apos;i Mania Region, Madagascar.</obo:IAO_0000115>
        <oboInOwl:hasOBONamespace>GAZ</oboInOwl:hasOBONamespace>
        <oboInOwl:id>GAZ:00076467</oboInOwl:id>
        <rdfs:label>Ambositra District</rdfs:label>
    </owl:NamedIndividual>
    


    <!-- http://purl.obolibrary.org/obo/GAZ_00076468 -->

    <owl:NamedIndividual rdf:about="http://purl.obolibrary.org/obo/GAZ_00076468">
        <rdf:type rdf:resource="http://purl.obolibrary.org/obo/ENVO_00000004"/>
        <obo:RO_0001025 rdf:resource="http://purl.obolibrary.org/obo/GAZ_00032058"/>
        <obo:IAO_0000115>A district in Haute Matsiatra Region, Madagascar.</obo:IAO_0000115>
        <oboInOwl:hasOBONamespace>GAZ</oboInOwl:hasOBONamespace>
        <oboInOwl:id>GAZ:00076468</oboInOwl:id>
        <rdfs:label>Ambohimahasoa District</rdfs:label>
    </owl:NamedIndividual>
    


    <!-- http://purl.obolibrary.org/obo/GAZ_00076469 -->

    <owl:NamedIndividual rdf:about="http://purl.obolibrary.org/obo/GAZ_00076469">
        <rdf:type rdf:resource="http://purl.obolibrary.org/obo/ENVO_00000004"/>
        <obo:RO_0001025 rdf:resource="http://purl.obolibrary.org/obo/GAZ_00032058"/>
        <obo:IAO_0000115>A district in Haute Matsiatra Region, Madagascar.</obo:IAO_0000115>
        <oboInOwl:hasOBONamespace>GAZ</oboInOwl:hasOBONamespace>
        <oboInOwl:id>GAZ:00076469</oboInOwl:id>
        <rdfs:label>Fianarantsoa District</rdfs:label>
    </owl:NamedIndividual>
    


    <!-- http://purl.obolibrary.org/obo/GAZ_00076470 -->

    <owl:NamedIndividual rdf:about="http://purl.obolibrary.org/obo/GAZ_00076470">
        <rdf:type rdf:resource="http://purl.obolibrary.org/obo/ENVO_00000004"/>
        <obo:RO_0001025 rdf:resource="http://purl.obolibrary.org/obo/GAZ_00032058"/>
        <obo:IAO_0000115>A district in Haute Matsiatra Region, Madagascar.</obo:IAO_0000115>
        <oboInOwl:hasOBONamespace>GAZ</oboInOwl:hasOBONamespace>
        <oboInOwl:id>GAZ:00076470</oboInOwl:id>
        <rdfs:label>Ikalamavony District</rdfs:label>
    </owl:NamedIndividual>
    


    <!-- http://purl.obolibrary.org/obo/GAZ_00076471 -->

    <owl:NamedIndividual rdf:about="http://purl.obolibrary.org/obo/GAZ_00076471">
        <rdf:type rdf:resource="http://purl.obolibrary.org/obo/ENVO_00000004"/>
        <obo:RO_0001025 rdf:resource="http://purl.obolibrary.org/obo/GAZ_00032058"/>
        <obo:IAO_0000115>A district in Haute Matsiatra Region, Madagascar.</obo:IAO_0000115>
        <oboInOwl:hasOBONamespace>GAZ</oboInOwl:hasOBONamespace>
        <oboInOwl:id>GAZ:00076471</oboInOwl:id>
        <rdfs:label>Ambalavao District</rdfs:label>
    </owl:NamedIndividual>
    


    <!-- http://purl.obolibrary.org/obo/GAZ_00076472 -->

    <owl:NamedIndividual rdf:about="http://purl.obolibrary.org/obo/GAZ_00076472">
        <rdf:type rdf:resource="http://purl.obolibrary.org/obo/ENVO_00000004"/>
        <obo:RO_0001025 rdf:resource="http://purl.obolibrary.org/obo/GAZ_00032058"/>
        <obo:IAO_0000115>A district in Haute Matsiatra Region, Madagascar.</obo:IAO_0000115>
        <oboInOwl:hasOBONamespace>GAZ</oboInOwl:hasOBONamespace>
        <oboInOwl:id>GAZ:00076472</oboInOwl:id>
        <rdfs:label>Fianarantsoa II District</rdfs:label>
    </owl:NamedIndividual>
    


    <!-- http://purl.obolibrary.org/obo/GAZ_00076473 -->

    <owl:NamedIndividual rdf:about="http://purl.obolibrary.org/obo/GAZ_00076473">
        <rdf:type rdf:resource="http://purl.obolibrary.org/obo/ENVO_00000004"/>
        <obo:RO_0001025 rdf:resource="http://purl.obolibrary.org/obo/GAZ_00032059"/>
        <obo:IAO_0000115>A district in Ihorombe Region, Madagascar.</obo:IAO_0000115>
        <oboInOwl:hasOBONamespace>GAZ</oboInOwl:hasOBONamespace>
        <oboInOwl:id>GAZ:00076473</oboInOwl:id>
        <rdfs:label>Ihosy District</rdfs:label>
    </owl:NamedIndividual>
    


    <!-- http://purl.obolibrary.org/obo/GAZ_00076474 -->

    <owl:NamedIndividual rdf:about="http://purl.obolibrary.org/obo/GAZ_00076474">
        <rdf:type rdf:resource="http://purl.obolibrary.org/obo/ENVO_00000004"/>
        <obo:RO_0001025 rdf:resource="http://purl.obolibrary.org/obo/GAZ_00032059"/>
        <obo:IAO_0000115>A district in Ihorombe Region, Madagascar.</obo:IAO_0000115>
        <oboInOwl:hasOBONamespace>GAZ</oboInOwl:hasOBONamespace>
        <oboInOwl:id>GAZ:00076474</oboInOwl:id>
        <rdfs:label>Iakora District</rdfs:label>
    </owl:NamedIndividual>
    


    <!-- http://purl.obolibrary.org/obo/GAZ_00076475 -->

    <owl:NamedIndividual rdf:about="http://purl.obolibrary.org/obo/GAZ_00076475">
        <rdf:type rdf:resource="http://purl.obolibrary.org/obo/ENVO_00000004"/>
        <obo:RO_0001025 rdf:resource="http://purl.obolibrary.org/obo/GAZ_00032059"/>
        <obo:IAO_0000115>A district in Ihorombe Region, Madagascar.</obo:IAO_0000115>
        <oboInOwl:hasOBONamespace>GAZ</oboInOwl:hasOBONamespace>
        <oboInOwl:id>GAZ:00076475</oboInOwl:id>
        <rdfs:label>Ivohibe District</rdfs:label>
    </owl:NamedIndividual>
    


    <!-- http://purl.obolibrary.org/obo/GAZ_00076476 -->

    <owl:NamedIndividual rdf:about="http://purl.obolibrary.org/obo/GAZ_00076476">
        <rdf:type rdf:resource="http://purl.obolibrary.org/obo/ENVO_00000004"/>
        <obo:RO_0001025 rdf:resource="http://purl.obolibrary.org/obo/GAZ_00032061"/>
        <obo:IAO_0000115>A district in Betsiboka Region, Madagascar.</obo:IAO_0000115>
        <oboInOwl:hasOBONamespace>GAZ</oboInOwl:hasOBONamespace>
        <oboInOwl:id>GAZ:00076476</oboInOwl:id>
        <rdfs:label>Maevatanana District</rdfs:label>
    </owl:NamedIndividual>
    


    <!-- http://purl.obolibrary.org/obo/GAZ_00076477 -->

    <owl:NamedIndividual rdf:about="http://purl.obolibrary.org/obo/GAZ_00076477">
        <rdf:type rdf:resource="http://purl.obolibrary.org/obo/ENVO_00000004"/>
        <obo:RO_0001025 rdf:resource="http://purl.obolibrary.org/obo/GAZ_00032061"/>
        <obo:IAO_0000115>A district in Betsiboka Region, Madagascar.</obo:IAO_0000115>
        <oboInOwl:hasOBONamespace>GAZ</oboInOwl:hasOBONamespace>
        <oboInOwl:id>GAZ:00076477</oboInOwl:id>
        <rdfs:label>Kandreho District</rdfs:label>
    </owl:NamedIndividual>
    


    <!-- http://purl.obolibrary.org/obo/GAZ_00076478 -->

    <owl:NamedIndividual rdf:about="http://purl.obolibrary.org/obo/GAZ_00076478">
        <rdf:type rdf:resource="http://purl.obolibrary.org/obo/ENVO_00000004"/>
        <obo:RO_0001025 rdf:resource="http://purl.obolibrary.org/obo/GAZ_00032061"/>
        <obo:IAO_0000115>A district in Betsiboka Region, Madagascar.</obo:IAO_0000115>
        <oboInOwl:hasOBONamespace>GAZ</oboInOwl:hasOBONamespace>
        <oboInOwl:id>GAZ:00076478</oboInOwl:id>
        <rdfs:label>Tsaratanana District</rdfs:label>
    </owl:NamedIndividual>
    


    <!-- http://purl.obolibrary.org/obo/GAZ_00076479 -->

    <owl:NamedIndividual rdf:about="http://purl.obolibrary.org/obo/GAZ_00076479">
        <rdf:type rdf:resource="http://purl.obolibrary.org/obo/ENVO_00000004"/>
        <obo:RO_0001025 rdf:resource="http://purl.obolibrary.org/obo/GAZ_00032062"/>
        <obo:IAO_0000115>A district in northwestern Madagascar. It&apos;s a part of Boeny Region of Mahajanga Province, and borders the districts of Mahajanga II in north, Boriziny and Mampikony in east, Ambato-Boeni in south and Mitsinjo in west.</obo:IAO_0000115>
        <oboInOwl:hasOBONamespace>GAZ</oboInOwl:hasOBONamespace>
        <oboInOwl:id>GAZ:00076479</oboInOwl:id>
        <rdfs:label>Marovoay District</rdfs:label>
    </owl:NamedIndividual>
    


    <!-- http://purl.obolibrary.org/obo/GAZ_00076480 -->

    <owl:NamedIndividual rdf:about="http://purl.obolibrary.org/obo/GAZ_00076480">
        <rdf:type rdf:resource="http://purl.obolibrary.org/obo/ENVO_00000004"/>
        <obo:RO_0001025 rdf:resource="http://purl.obolibrary.org/obo/GAZ_00032062"/>
        <obo:IAO_0000115>A district in western Madagascar. It&apos;s a part of Boeny Region of Mahajanga Province, and borders the districts of Mitsinjo in northeast, Ambato-Boeni in east, Kandreho in south and Besalampy in west.</obo:IAO_0000115>
        <oboInOwl:hasOBONamespace>GAZ</oboInOwl:hasOBONamespace>
        <oboInOwl:id>GAZ:00076480</oboInOwl:id>
        <rdfs:label>Soalala District</rdfs:label>
    </owl:NamedIndividual>
    


    <!-- http://purl.obolibrary.org/obo/GAZ_00076481 -->

    <owl:NamedIndividual rdf:about="http://purl.obolibrary.org/obo/GAZ_00076481">
        <rdf:type rdf:resource="http://purl.obolibrary.org/obo/ENVO_00000004"/>
        <obo:RO_0001025 rdf:resource="http://purl.obolibrary.org/obo/GAZ_00032062"/>
        <obo:IAO_0000115>A district in western Madagascar. It&apos;s a part of Boeny Region of Mahajanga Province, and borders the districts of Marovoay in east, Ambato-Boeni in south and Soalala in west.</obo:IAO_0000115>
        <oboInOwl:hasOBONamespace>GAZ</oboInOwl:hasOBONamespace>
        <oboInOwl:id>GAZ:00076481</oboInOwl:id>
        <rdfs:label>Mitsinjo District</rdfs:label>
    </owl:NamedIndividual>
    


    <!-- http://purl.obolibrary.org/obo/GAZ_00076482 -->

    <owl:NamedIndividual rdf:about="http://purl.obolibrary.org/obo/GAZ_00076482">
        <rdf:type rdf:resource="http://purl.obolibrary.org/obo/ENVO_00000004"/>
        <obo:RO_0001025 rdf:resource="http://purl.obolibrary.org/obo/GAZ_00032062"/>
        <obo:IAO_0000115>A district in Boeny Region, Madagascar.</obo:IAO_0000115>
        <oboInOwl:hasOBONamespace>GAZ</oboInOwl:hasOBONamespace>
        <oboInOwl:id>GAZ:00076482</oboInOwl:id>
        <rdfs:label>Mahajanga I District</rdfs:label>
    </owl:NamedIndividual>
    


    <!-- http://purl.obolibrary.org/obo/GAZ_00076483 -->

    <owl:NamedIndividual rdf:about="http://purl.obolibrary.org/obo/GAZ_00076483">
        <rdf:type rdf:resource="http://purl.obolibrary.org/obo/ENVO_00000004"/>
        <obo:RO_0001025 rdf:resource="http://purl.obolibrary.org/obo/GAZ_00032062"/>
        <obo:IAO_0000115>A district in Boeny Region, Madagascar. It surrounds Mahajanga I.</obo:IAO_0000115>
        <oboInOwl:hasOBONamespace>GAZ</oboInOwl:hasOBONamespace>
        <oboInOwl:id>GAZ:00076483</oboInOwl:id>
        <rdfs:label>Mahajanga II District</rdfs:label>
    </owl:NamedIndividual>
    


    <!-- http://purl.obolibrary.org/obo/GAZ_00076484 -->

    <owl:NamedIndividual rdf:about="http://purl.obolibrary.org/obo/GAZ_00076484">
        <rdf:type rdf:resource="http://purl.obolibrary.org/obo/ENVO_00000004"/>
        <obo:RO_0001025 rdf:resource="http://purl.obolibrary.org/obo/GAZ_00032062"/>
        <obo:IAO_0000115>A district in Boeny Region, Madagascar.</obo:IAO_0000115>
        <oboInOwl:hasOBONamespace>GAZ</oboInOwl:hasOBONamespace>
        <oboInOwl:id>GAZ:00076484</oboInOwl:id>
        <rdfs:label>Ambato-Boeni District</rdfs:label>
    </owl:NamedIndividual>
    


    <!-- http://purl.obolibrary.org/obo/GAZ_00076485 -->

    <owl:NamedIndividual rdf:about="http://purl.obolibrary.org/obo/GAZ_00076485">
        <rdf:type rdf:resource="http://purl.obolibrary.org/obo/ENVO_00000004"/>
        <obo:RO_0001025 rdf:resource="http://purl.obolibrary.org/obo/GAZ_00032063"/>
        <obo:IAO_0000115>A district in western Madagascar. It&apos;s a part of Melaky Region of Mahajanga Province, and borders the districts of Besalampy in north, Morafenobe in east and Antsalova in south.</obo:IAO_0000115>
        <oboInOwl:hasOBONamespace>GAZ</oboInOwl:hasOBONamespace>
        <oboInOwl:id>GAZ:00076485</oboInOwl:id>
        <rdfs:label>Maintirano District</rdfs:label>
    </owl:NamedIndividual>
    


    <!-- http://purl.obolibrary.org/obo/GAZ_00076486 -->

    <owl:NamedIndividual rdf:about="http://purl.obolibrary.org/obo/GAZ_00076486">
        <rdf:type rdf:resource="http://purl.obolibrary.org/obo/ENVO_00000004"/>
        <obo:RO_0001025 rdf:resource="http://purl.obolibrary.org/obo/GAZ_00032063"/>
        <obo:IAO_0000115>A district in western Madagascar. It&apos;s a part of Melaky Region of Mahajanga Province, and borders the districts of Maintirano in north, Morafenobe in northeast, Miandrivazo in east and Belon&apos;i Tsiribihina in south.</obo:IAO_0000115>
        <oboInOwl:hasOBONamespace>GAZ</oboInOwl:hasOBONamespace>
        <oboInOwl:id>GAZ:00076486</oboInOwl:id>
        <rdfs:label>Antsalova District</rdfs:label>
    </owl:NamedIndividual>
    


    <!-- http://purl.obolibrary.org/obo/GAZ_00076487 -->

    <owl:NamedIndividual rdf:about="http://purl.obolibrary.org/obo/GAZ_00076487">
        <rdf:type rdf:resource="http://purl.obolibrary.org/obo/ENVO_00000004"/>
        <obo:RO_0001025 rdf:resource="http://purl.obolibrary.org/obo/GAZ_00032063"/>
        <obo:IAO_0000115>A district in western Madagascar. It&apos;s a part of Melaky Region of Mahajanga Province, and borders the districts of Besalampy in north, Ambatomainty in east, Miandrivazo in south, Antsalova in southwest and Maintirano in west.</obo:IAO_0000115>
        <oboInOwl:hasOBONamespace>GAZ</oboInOwl:hasOBONamespace>
        <oboInOwl:id>GAZ:00076487</oboInOwl:id>
        <rdfs:label>Morafenobe District</rdfs:label>
    </owl:NamedIndividual>
    


    <!-- http://purl.obolibrary.org/obo/GAZ_00076488 -->

    <owl:NamedIndividual rdf:about="http://purl.obolibrary.org/obo/GAZ_00076488">
        <rdf:type rdf:resource="http://purl.obolibrary.org/obo/ENVO_00000004"/>
        <obo:RO_0001025 rdf:resource="http://purl.obolibrary.org/obo/GAZ_00032063"/>
        <obo:IAO_0000115>A district in western Madagascar. It&apos;s a part of Melaky Region of Mahajanga Province, and borders the districts of Soalala in northeast, Kandreho in east, Ambatomainty in southeast, Morafenobe in south and Maintirano in southwest.</obo:IAO_0000115>
        <oboInOwl:hasOBONamespace>GAZ</oboInOwl:hasOBONamespace>
        <oboInOwl:id>GAZ:00076488</oboInOwl:id>
        <rdfs:label>Besalampy District</rdfs:label>
    </owl:NamedIndividual>
    


    <!-- http://purl.obolibrary.org/obo/GAZ_00076489 -->

    <owl:NamedIndividual rdf:about="http://purl.obolibrary.org/obo/GAZ_00076489">
        <rdf:type rdf:resource="http://purl.obolibrary.org/obo/ENVO_00000004"/>
        <obo:RO_0001025 rdf:resource="http://purl.obolibrary.org/obo/GAZ_00032064"/>
        <obo:IAO_0000115>A district in Sofia Region, Madagascar.</obo:IAO_0000115>
        <oboInOwl:hasOBONamespace>GAZ</oboInOwl:hasOBONamespace>
        <oboInOwl:id>GAZ:00076489</oboInOwl:id>
        <rdfs:label>Antsohihy District</rdfs:label>
    </owl:NamedIndividual>
    


    <!-- http://purl.obolibrary.org/obo/GAZ_00076490 -->

    <owl:NamedIndividual rdf:about="http://purl.obolibrary.org/obo/GAZ_00076490">
        <rdf:type rdf:resource="http://purl.obolibrary.org/obo/ENVO_00000004"/>
        <obo:RO_0001025 rdf:resource="http://purl.obolibrary.org/obo/GAZ_00032064"/>
        <obo:IAO_0000115>A district in Sofia Region, Madagascar.</obo:IAO_0000115>
        <oboInOwl:hasOBONamespace>GAZ</oboInOwl:hasOBONamespace>
        <oboInOwl:id>GAZ:00076490</oboInOwl:id>
        <rdfs:label>Mandritsara District</rdfs:label>
    </owl:NamedIndividual>
    


    <!-- http://purl.obolibrary.org/obo/GAZ_00076491 -->

    <owl:NamedIndividual rdf:about="http://purl.obolibrary.org/obo/GAZ_00076491">
        <rdf:type rdf:resource="http://purl.obolibrary.org/obo/ENVO_00000004"/>
        <obo:RO_0001025 rdf:resource="http://purl.obolibrary.org/obo/GAZ_00032064"/>
        <obo:IAO_0000115>A district in Sofia Region, Madagascar.</obo:IAO_0000115>
        <oboInOwl:hasOBONamespace>GAZ</oboInOwl:hasOBONamespace>
        <oboInOwl:id>GAZ:00076491</oboInOwl:id>
        <rdfs:label>Befandriana avaratra District</rdfs:label>
    </owl:NamedIndividual>
    


    <!-- http://purl.obolibrary.org/obo/GAZ_00076492 -->

    <owl:NamedIndividual rdf:about="http://purl.obolibrary.org/obo/GAZ_00076492">
        <rdf:type rdf:resource="http://purl.obolibrary.org/obo/ENVO_00000004"/>
        <obo:RO_0001025 rdf:resource="http://purl.obolibrary.org/obo/GAZ_00032064"/>
        <obo:IAO_0000115>A district in Sofia Region, Madagascar.</obo:IAO_0000115>
        <oboInOwl:hasOBONamespace>GAZ</oboInOwl:hasOBONamespace>
        <oboInOwl:id>GAZ:00076492</oboInOwl:id>
        <rdfs:label>Mampikony District</rdfs:label>
    </owl:NamedIndividual>
    


    <!-- http://purl.obolibrary.org/obo/GAZ_00076493 -->

    <owl:NamedIndividual rdf:about="http://purl.obolibrary.org/obo/GAZ_00076493">
        <rdf:type rdf:resource="http://purl.obolibrary.org/obo/ENVO_00000004"/>
        <obo:RO_0001025 rdf:resource="http://purl.obolibrary.org/obo/GAZ_00032064"/>
        <obo:IAO_0000115>A district in Sofia Region, Madagascar.</obo:IAO_0000115>
        <oboInOwl:hasOBONamespace>GAZ</oboInOwl:hasOBONamespace>
        <oboInOwl:id>GAZ:00076493</oboInOwl:id>
        <rdfs:label>Analalava District</rdfs:label>
    </owl:NamedIndividual>
    


    <!-- http://purl.obolibrary.org/obo/GAZ_00076494 -->

    <owl:NamedIndividual rdf:about="http://purl.obolibrary.org/obo/GAZ_00076494">
        <rdf:type rdf:resource="http://purl.obolibrary.org/obo/ENVO_00000004"/>
        <obo:RO_0001025 rdf:resource="http://purl.obolibrary.org/obo/GAZ_00032064"/>
        <obo:IAO_0000115>A district in Sofia Region, Madagascar.</obo:IAO_0000115>
        <oboInOwl:hasOBONamespace>GAZ</oboInOwl:hasOBONamespace>
        <oboInOwl:id>GAZ:00076494</oboInOwl:id>
        <rdfs:label>Bealanana District</rdfs:label>
    </owl:NamedIndividual>
    


    <!-- http://purl.obolibrary.org/obo/GAZ_00076495 -->

    <owl:NamedIndividual rdf:about="http://purl.obolibrary.org/obo/GAZ_00076495">
        <rdf:type rdf:resource="http://purl.obolibrary.org/obo/ENVO_00000004"/>
        <obo:RO_0001025 rdf:resource="http://purl.obolibrary.org/obo/GAZ_00032064"/>
        <obo:IAO_0000115>A district in Sofia Region, Madagascar.</obo:IAO_0000115>
        <oboInOwl:hasOBONamespace>GAZ</oboInOwl:hasOBONamespace>
        <oboInOwl:id>GAZ:00076495</oboInOwl:id>
        <rdfs:label>Port-Berge District</rdfs:label>
    </owl:NamedIndividual>
    


    <!-- http://purl.obolibrary.org/obo/GAZ_00076496 -->

    <owl:NamedIndividual rdf:about="http://purl.obolibrary.org/obo/GAZ_00076496">
        <rdf:type rdf:resource="http://purl.obolibrary.org/obo/ENVO_00000004"/>
        <obo:RO_0001025 rdf:resource="http://purl.obolibrary.org/obo/GAZ_00032065"/>
        <obo:IAO_0000115>A district in Alaotra Mangoro Region, Madagascar.</obo:IAO_0000115>
        <oboInOwl:hasOBONamespace>GAZ</oboInOwl:hasOBONamespace>
        <oboInOwl:id>GAZ:00076496</oboInOwl:id>
        <rdfs:label>Amparafaravola District</rdfs:label>
    </owl:NamedIndividual>
    


    <!-- http://purl.obolibrary.org/obo/GAZ_00076497 -->

    <owl:NamedIndividual rdf:about="http://purl.obolibrary.org/obo/GAZ_00076497">
        <rdf:type rdf:resource="http://purl.obolibrary.org/obo/ENVO_00000004"/>
        <obo:RO_0001025 rdf:resource="http://purl.obolibrary.org/obo/GAZ_00032065"/>
        <obo:IAO_0000115>A district in Alaotra Mangoro Region, Madagascar.</obo:IAO_0000115>
        <oboInOwl:hasOBONamespace>GAZ</oboInOwl:hasOBONamespace>
        <oboInOwl:id>GAZ:00076497</oboInOwl:id>
        <rdfs:label>Anosibe An&apos;ala District</rdfs:label>
    </owl:NamedIndividual>
    


    <!-- http://purl.obolibrary.org/obo/GAZ_00076498 -->

    <owl:NamedIndividual rdf:about="http://purl.obolibrary.org/obo/GAZ_00076498">
        <rdf:type rdf:resource="http://purl.obolibrary.org/obo/ENVO_00000004"/>
        <obo:RO_0001025 rdf:resource="http://purl.obolibrary.org/obo/GAZ_00032065"/>
        <obo:IAO_0000115>A district in Alaotra Mangoro Region, Madagascar.</obo:IAO_0000115>
        <oboInOwl:hasOBONamespace>GAZ</oboInOwl:hasOBONamespace>
        <oboInOwl:id>GAZ:00076498</oboInOwl:id>
        <rdfs:label>Moramanga District</rdfs:label>
    </owl:NamedIndividual>
    


    <!-- http://purl.obolibrary.org/obo/GAZ_00076499 -->

    <owl:NamedIndividual rdf:about="http://purl.obolibrary.org/obo/GAZ_00076499">
        <rdf:type rdf:resource="http://purl.obolibrary.org/obo/ENVO_00000004"/>
        <obo:RO_0001025 rdf:resource="http://purl.obolibrary.org/obo/GAZ_00032065"/>
        <obo:IAO_0000115>A district in Alaotra Mangoro Region, Madagascar.</obo:IAO_0000115>
        <oboInOwl:hasOBONamespace>GAZ</oboInOwl:hasOBONamespace>
        <oboInOwl:id>GAZ:00076499</oboInOwl:id>
        <rdfs:label>Ambatondrazaka District</rdfs:label>
    </owl:NamedIndividual>
    


    <!-- http://purl.obolibrary.org/obo/GAZ_00076500 -->

    <owl:NamedIndividual rdf:about="http://purl.obolibrary.org/obo/GAZ_00076500">
        <rdf:type rdf:resource="http://purl.obolibrary.org/obo/ENVO_00000004"/>
        <obo:RO_0001025 rdf:resource="http://purl.obolibrary.org/obo/GAZ_00032065"/>
        <obo:IAO_0000115>A district in Alaotra Mangoro Region, Madagascar.</obo:IAO_0000115>
        <oboInOwl:hasOBONamespace>GAZ</oboInOwl:hasOBONamespace>
        <oboInOwl:id>GAZ:00076500</oboInOwl:id>
        <rdfs:label>Andilamena District</rdfs:label>
    </owl:NamedIndividual>
    


    <!-- http://purl.obolibrary.org/obo/GAZ_00076501 -->

    <owl:NamedIndividual rdf:about="http://purl.obolibrary.org/obo/GAZ_00076501">
        <rdf:type rdf:resource="http://purl.obolibrary.org/obo/ENVO_00000004"/>
        <obo:RO_0001025 rdf:resource="http://purl.obolibrary.org/obo/GAZ_00032066"/>
        <obo:IAO_0000115>A district in Analanjirofo Region, Madagascar.</obo:IAO_0000115>
        <oboInOwl:hasOBONamespace>GAZ</oboInOwl:hasOBONamespace>
        <oboInOwl:id>GAZ:00076501</oboInOwl:id>
        <rdfs:label>Maroantsetra District</rdfs:label>
    </owl:NamedIndividual>
    


    <!-- http://purl.obolibrary.org/obo/GAZ_00076502 -->

    <owl:NamedIndividual rdf:about="http://purl.obolibrary.org/obo/GAZ_00076502">
        <rdf:type rdf:resource="http://purl.obolibrary.org/obo/ENVO_00000004"/>
        <obo:RO_0001025 rdf:resource="http://purl.obolibrary.org/obo/GAZ_00032066"/>
        <obo:IAO_0000115>A district in Analanjirofo Region, Madagascar.</obo:IAO_0000115>
        <oboInOwl:hasOBONamespace>GAZ</oboInOwl:hasOBONamespace>
        <oboInOwl:id>GAZ:00076502</oboInOwl:id>
        <rdfs:label>Vavatenina District</rdfs:label>
    </owl:NamedIndividual>
    


    <!-- http://purl.obolibrary.org/obo/GAZ_00076503 -->

    <owl:NamedIndividual rdf:about="http://purl.obolibrary.org/obo/GAZ_00076503">
        <rdf:type rdf:resource="http://purl.obolibrary.org/obo/ENVO_00000004"/>
        <obo:RO_0001025 rdf:resource="http://purl.obolibrary.org/obo/GAZ_00032066"/>
        <obo:IAO_0000115>A district in Analanjirofo Region, Madagascar.</obo:IAO_0000115>
        <oboInOwl:hasOBONamespace>GAZ</oboInOwl:hasOBONamespace>
        <oboInOwl:id>GAZ:00076503</oboInOwl:id>
        <rdfs:label>Sainte Marie District</rdfs:label>
    </owl:NamedIndividual>
    


    <!-- http://purl.obolibrary.org/obo/GAZ_00076504 -->

    <owl:NamedIndividual rdf:about="http://purl.obolibrary.org/obo/GAZ_00076504">
        <rdf:type rdf:resource="http://purl.obolibrary.org/obo/ENVO_00000004"/>
        <obo:RO_0001025 rdf:resource="http://purl.obolibrary.org/obo/GAZ_00032066"/>
        <obo:IAO_0000115>A district in Analanjirofo Region, Madagascar.</obo:IAO_0000115>
        <oboInOwl:hasOBONamespace>GAZ</oboInOwl:hasOBONamespace>
        <oboInOwl:id>GAZ:00076504</oboInOwl:id>
        <rdfs:label>Soanierana Ivongo District</rdfs:label>
    </owl:NamedIndividual>
    


    <!-- http://purl.obolibrary.org/obo/GAZ_00076505 -->

    <owl:NamedIndividual rdf:about="http://purl.obolibrary.org/obo/GAZ_00076505">
        <rdf:type rdf:resource="http://purl.obolibrary.org/obo/ENVO_00000004"/>
        <obo:RO_0001025 rdf:resource="http://purl.obolibrary.org/obo/GAZ_00032066"/>
        <obo:IAO_0000115>A district in Analanjirofo Region, Madagascar.</obo:IAO_0000115>
        <oboInOwl:hasOBONamespace>GAZ</oboInOwl:hasOBONamespace>
        <oboInOwl:id>GAZ:00076505</oboInOwl:id>
        <rdfs:label>Mananara Nord District</rdfs:label>
    </owl:NamedIndividual>
    


    <!-- http://purl.obolibrary.org/obo/GAZ_00076506 -->

    <owl:NamedIndividual rdf:about="http://purl.obolibrary.org/obo/GAZ_00076506">
        <rdf:type rdf:resource="http://purl.obolibrary.org/obo/ENVO_00000004"/>
        <obo:RO_0001025 rdf:resource="http://purl.obolibrary.org/obo/GAZ_00032066"/>
        <obo:IAO_0000115>A district in Analanjirofo Region, Madagascar.</obo:IAO_0000115>
        <oboInOwl:hasOBONamespace>GAZ</oboInOwl:hasOBONamespace>
        <oboInOwl:id>GAZ:00076506</oboInOwl:id>
        <rdfs:label>Fenerive Est District</rdfs:label>
    </owl:NamedIndividual>
    


    <!-- http://purl.obolibrary.org/obo/GAZ_00076507 -->

    <owl:NamedIndividual rdf:about="http://purl.obolibrary.org/obo/GAZ_00076507">
        <rdf:type rdf:resource="http://purl.obolibrary.org/obo/ENVO_00000004"/>
        <obo:RO_0001025 rdf:resource="http://purl.obolibrary.org/obo/GAZ_00032067"/>
        <obo:IAO_0000115>A district in Atsinanana Region, Madagascar.</obo:IAO_0000115>
        <oboInOwl:hasOBONamespace>GAZ</oboInOwl:hasOBONamespace>
        <oboInOwl:id>GAZ:00076507</oboInOwl:id>
        <rdfs:label>Vatomandry District</rdfs:label>
    </owl:NamedIndividual>
    


    <!-- http://purl.obolibrary.org/obo/GAZ_00076508 -->

    <owl:NamedIndividual rdf:about="http://purl.obolibrary.org/obo/GAZ_00076508">
        <rdf:type rdf:resource="http://purl.obolibrary.org/obo/ENVO_00000004"/>
        <obo:RO_0001025 rdf:resource="http://purl.obolibrary.org/obo/GAZ_00032067"/>
        <obo:IAO_0000115>A district in Atsinanana Region, Madagascar.</obo:IAO_0000115>
        <oboInOwl:hasOBONamespace>GAZ</oboInOwl:hasOBONamespace>
        <oboInOwl:id>GAZ:00076508</oboInOwl:id>
        <rdfs:label>Marolambo District</rdfs:label>
    </owl:NamedIndividual>
    


    <!-- http://purl.obolibrary.org/obo/GAZ_00076509 -->

    <owl:NamedIndividual rdf:about="http://purl.obolibrary.org/obo/GAZ_00076509">
        <rdf:type rdf:resource="http://purl.obolibrary.org/obo/ENVO_00000004"/>
        <obo:RO_0001025 rdf:resource="http://purl.obolibrary.org/obo/GAZ_00032067"/>
        <obo:IAO_0000115>A district in Atsinanana Region, Madagascar.</obo:IAO_0000115>
        <oboInOwl:hasOBONamespace>GAZ</oboInOwl:hasOBONamespace>
        <oboInOwl:id>GAZ:00076509</oboInOwl:id>
        <rdfs:label>Toamasina District</rdfs:label>
    </owl:NamedIndividual>
    


    <!-- http://purl.obolibrary.org/obo/GAZ_00076510 -->

    <owl:NamedIndividual rdf:about="http://purl.obolibrary.org/obo/GAZ_00076510">
        <rdf:type rdf:resource="http://purl.obolibrary.org/obo/ENVO_00000004"/>
        <obo:RO_0001025 rdf:resource="http://purl.obolibrary.org/obo/GAZ_00032067"/>
        <obo:IAO_0000115>A district in Atsinanana Region, Madagascar.</obo:IAO_0000115>
        <oboInOwl:hasOBONamespace>GAZ</oboInOwl:hasOBONamespace>
        <oboInOwl:id>GAZ:00076510</oboInOwl:id>
        <rdfs:label>Toamasina II District</rdfs:label>
    </owl:NamedIndividual>
    


    <!-- http://purl.obolibrary.org/obo/GAZ_00076511 -->

    <owl:NamedIndividual rdf:about="http://purl.obolibrary.org/obo/GAZ_00076511">
        <rdf:type rdf:resource="http://purl.obolibrary.org/obo/ENVO_00000004"/>
        <obo:RO_0001025 rdf:resource="http://purl.obolibrary.org/obo/GAZ_00032067"/>
        <obo:IAO_0000115>A district in Atsinanana Region, Madagascar.</obo:IAO_0000115>
        <oboInOwl:hasOBONamespace>GAZ</oboInOwl:hasOBONamespace>
        <oboInOwl:id>GAZ:00076511</oboInOwl:id>
        <rdfs:label>Brickaville District</rdfs:label>
    </owl:NamedIndividual>
    


    <!-- http://purl.obolibrary.org/obo/GAZ_00076512 -->

    <owl:NamedIndividual rdf:about="http://purl.obolibrary.org/obo/GAZ_00076512">
        <rdf:type rdf:resource="http://purl.obolibrary.org/obo/ENVO_00000004"/>
        <obo:RO_0001025 rdf:resource="http://purl.obolibrary.org/obo/GAZ_00032067"/>
        <obo:IAO_0000115>A district in Atsinanana Region, Madagascar.</obo:IAO_0000115>
        <oboInOwl:hasOBONamespace>GAZ</oboInOwl:hasOBONamespace>
        <oboInOwl:id>GAZ:00076512</oboInOwl:id>
        <rdfs:label>Antanambao Manampotsy District</rdfs:label>
    </owl:NamedIndividual>
    


    <!-- http://purl.obolibrary.org/obo/GAZ_00076513 -->

    <owl:NamedIndividual rdf:about="http://purl.obolibrary.org/obo/GAZ_00076513">
        <rdf:type rdf:resource="http://purl.obolibrary.org/obo/ENVO_00000004"/>
        <obo:RO_0001025 rdf:resource="http://purl.obolibrary.org/obo/GAZ_00032067"/>
        <obo:IAO_0000115>A district in Atsinanana Region, Madagascar.</obo:IAO_0000115>
        <oboInOwl:hasOBONamespace>GAZ</oboInOwl:hasOBONamespace>
        <oboInOwl:id>GAZ:00076513</oboInOwl:id>
        <rdfs:label>Mahanoro District</rdfs:label>
    </owl:NamedIndividual>
    


    <!-- http://purl.obolibrary.org/obo/GAZ_00076514 -->

    <owl:NamedIndividual rdf:about="http://purl.obolibrary.org/obo/GAZ_00076514">
        <rdf:type rdf:resource="http://purl.obolibrary.org/obo/ENVO_00000004"/>
        <obo:RO_0001025 rdf:resource="http://purl.obolibrary.org/obo/GAZ_00032069"/>
        <obo:IAO_0000115>A district in Anosy Region, Madagascar.</obo:IAO_0000115>
        <oboInOwl:hasOBONamespace>GAZ</oboInOwl:hasOBONamespace>
        <oboInOwl:id>GAZ:00076514</oboInOwl:id>
        <rdfs:label>Amboasary Sud District</rdfs:label>
    </owl:NamedIndividual>
    


    <!-- http://purl.obolibrary.org/obo/GAZ_00076515 -->

    <owl:NamedIndividual rdf:about="http://purl.obolibrary.org/obo/GAZ_00076515">
        <rdf:type rdf:resource="http://purl.obolibrary.org/obo/ENVO_00000004"/>
        <obo:RO_0001025 rdf:resource="http://purl.obolibrary.org/obo/GAZ_00032069"/>
        <obo:IAO_0000115>A district in Anosy Region, Madagascar.</obo:IAO_0000115>
        <oboInOwl:hasOBONamespace>GAZ</oboInOwl:hasOBONamespace>
        <oboInOwl:id>GAZ:00076515</oboInOwl:id>
        <rdfs:label>Betroka District</rdfs:label>
    </owl:NamedIndividual>
    


    <!-- http://purl.obolibrary.org/obo/GAZ_00076516 -->

    <owl:NamedIndividual rdf:about="http://purl.obolibrary.org/obo/GAZ_00076516">
        <rdf:type rdf:resource="http://purl.obolibrary.org/obo/ENVO_00000004"/>
        <obo:RO_0001025 rdf:resource="http://purl.obolibrary.org/obo/GAZ_00032069"/>
        <obo:IAO_0000115>A district in Anosy Region, Madagascar.</obo:IAO_0000115>
        <oboInOwl:hasOBONamespace>GAZ</oboInOwl:hasOBONamespace>
        <oboInOwl:id>GAZ:00076516</oboInOwl:id>
        <rdfs:label>Tolanaro District</rdfs:label>
    </owl:NamedIndividual>
    


    <!-- http://purl.obolibrary.org/obo/GAZ_00076517 -->

    <owl:NamedIndividual rdf:about="http://purl.obolibrary.org/obo/GAZ_00076517">
        <rdf:type rdf:resource="http://purl.obolibrary.org/obo/ENVO_00000004"/>
        <obo:RO_0001025 rdf:resource="http://purl.obolibrary.org/obo/GAZ_00032070"/>
        <obo:IAO_0000115>A district in Atsimo-Andrefana Region, Madagascar.</obo:IAO_0000115>
        <oboInOwl:hasOBONamespace>GAZ</oboInOwl:hasOBONamespace>
        <oboInOwl:id>GAZ:00076517</oboInOwl:id>
        <rdfs:label>Ampanihy District</rdfs:label>
    </owl:NamedIndividual>
    


    <!-- http://purl.obolibrary.org/obo/GAZ_00076518 -->

    <owl:NamedIndividual rdf:about="http://purl.obolibrary.org/obo/GAZ_00076518">
        <rdf:type rdf:resource="http://purl.obolibrary.org/obo/ENVO_00000004"/>
        <obo:RO_0001025 rdf:resource="http://purl.obolibrary.org/obo/GAZ_00032070"/>
        <obo:IAO_0000115>A district in Atsimo-Andrefana Region, Madagascar.</obo:IAO_0000115>
        <oboInOwl:hasOBONamespace>GAZ</oboInOwl:hasOBONamespace>
        <oboInOwl:id>GAZ:00076518</oboInOwl:id>
        <rdfs:label>Ankazoabo District</rdfs:label>
    </owl:NamedIndividual>
    


    <!-- http://purl.obolibrary.org/obo/GAZ_00076519 -->

    <owl:NamedIndividual rdf:about="http://purl.obolibrary.org/obo/GAZ_00076519">
        <rdf:type rdf:resource="http://purl.obolibrary.org/obo/ENVO_00000004"/>
        <obo:RO_0001025 rdf:resource="http://purl.obolibrary.org/obo/GAZ_00032070"/>
        <obo:IAO_0000115>A district in Atsimo-Andrefana Region, Madagascar.</obo:IAO_0000115>
        <oboInOwl:hasOBONamespace>GAZ</oboInOwl:hasOBONamespace>
        <oboInOwl:id>GAZ:00076519</oboInOwl:id>
        <rdfs:label>Morombe District</rdfs:label>
    </owl:NamedIndividual>
    


    <!-- http://purl.obolibrary.org/obo/GAZ_00076520 -->

    <owl:NamedIndividual rdf:about="http://purl.obolibrary.org/obo/GAZ_00076520">
        <rdf:type rdf:resource="http://purl.obolibrary.org/obo/ENVO_00000004"/>
        <obo:RO_0001025 rdf:resource="http://purl.obolibrary.org/obo/GAZ_00032070"/>
        <obo:IAO_0000115>A district in Atsimo-Andrefana Region, Madagascar.</obo:IAO_0000115>
        <oboInOwl:hasOBONamespace>GAZ</oboInOwl:hasOBONamespace>
        <oboInOwl:id>GAZ:00076520</oboInOwl:id>
        <rdfs:label>Benenitra District</rdfs:label>
    </owl:NamedIndividual>
    


    <!-- http://purl.obolibrary.org/obo/GAZ_00076521 -->

    <owl:NamedIndividual rdf:about="http://purl.obolibrary.org/obo/GAZ_00076521">
        <rdf:type rdf:resource="http://purl.obolibrary.org/obo/ENVO_00000004"/>
        <obo:RO_0001025 rdf:resource="http://purl.obolibrary.org/obo/GAZ_00032070"/>
        <obo:IAO_0000115>A district in Atsimo-Andrefana Region, Madagascar.</obo:IAO_0000115>
        <oboInOwl:hasOBONamespace>GAZ</oboInOwl:hasOBONamespace>
        <oboInOwl:id>GAZ:00076521</oboInOwl:id>
        <rdfs:label>Beroroha District</rdfs:label>
    </owl:NamedIndividual>
    


    <!-- http://purl.obolibrary.org/obo/GAZ_00076522 -->

    <owl:NamedIndividual rdf:about="http://purl.obolibrary.org/obo/GAZ_00076522">
        <rdf:type rdf:resource="http://purl.obolibrary.org/obo/ENVO_00000004"/>
        <obo:RO_0001025 rdf:resource="http://purl.obolibrary.org/obo/GAZ_00032070"/>
        <obo:IAO_0000115>A district in Atsimo-Andrefana Region, Madagascar.</obo:IAO_0000115>
        <oboInOwl:hasOBONamespace>GAZ</oboInOwl:hasOBONamespace>
        <oboInOwl:id>GAZ:00076522</oboInOwl:id>
        <rdfs:label>Betioky Sud District</rdfs:label>
    </owl:NamedIndividual>
    


    <!-- http://purl.obolibrary.org/obo/GAZ_00076523 -->

    <owl:NamedIndividual rdf:about="http://purl.obolibrary.org/obo/GAZ_00076523">
        <rdf:type rdf:resource="http://purl.obolibrary.org/obo/ENVO_00000004"/>
        <obo:RO_0001025 rdf:resource="http://purl.obolibrary.org/obo/GAZ_00032070"/>
        <obo:IAO_0000115>A district in Atsimo-Andrefana Region, Madagascar.</obo:IAO_0000115>
        <oboInOwl:hasOBONamespace>GAZ</oboInOwl:hasOBONamespace>
        <oboInOwl:id>GAZ:00076523</oboInOwl:id>
        <rdfs:label>Sakaraha District</rdfs:label>
    </owl:NamedIndividual>
    


    <!-- http://purl.obolibrary.org/obo/GAZ_00076524 -->

    <owl:NamedIndividual rdf:about="http://purl.obolibrary.org/obo/GAZ_00076524">
        <rdf:type rdf:resource="http://purl.obolibrary.org/obo/ENVO_00000004"/>
        <obo:RO_0001025 rdf:resource="http://purl.obolibrary.org/obo/GAZ_00032070"/>
        <obo:IAO_0000115>A district in Atsimo-Andrefana Region, Madagascar.</obo:IAO_0000115>
        <oboInOwl:hasOBONamespace>GAZ</oboInOwl:hasOBONamespace>
        <oboInOwl:id>GAZ:00076524</oboInOwl:id>
        <rdfs:label>Toliara II District</rdfs:label>
    </owl:NamedIndividual>
    


    <!-- http://purl.obolibrary.org/obo/GAZ_00076525 -->

    <owl:NamedIndividual rdf:about="http://purl.obolibrary.org/obo/GAZ_00076525">
        <rdf:type rdf:resource="http://purl.obolibrary.org/obo/ENVO_00000004"/>
        <obo:RO_0001025 rdf:resource="http://purl.obolibrary.org/obo/GAZ_00032070"/>
        <obo:IAO_0000115>A district in Atsimo-Andrefana Region, Madagascar.</obo:IAO_0000115>
        <oboInOwl:hasOBONamespace>GAZ</oboInOwl:hasOBONamespace>
        <oboInOwl:id>GAZ:00076525</oboInOwl:id>
        <rdfs:label>Toliara District</rdfs:label>
    </owl:NamedIndividual>
    


    <!-- http://purl.obolibrary.org/obo/GAZ_00076526 -->

    <owl:NamedIndividual rdf:about="http://purl.obolibrary.org/obo/GAZ_00076526">
        <obo:RO_0001025 rdf:resource="http://purl.obolibrary.org/obo/GAZ_00032070"/>
        <obo:IAO_0000115>A protected area located at 35 km northeast of Betioky Sud and 100 km inland from Toliara in the Southwest of Madagascar.</obo:IAO_0000115>
        <oboInOwl:hasOBONamespace>GAZ</oboInOwl:hasOBONamespace>
        <oboInOwl:id>GAZ:00076526</oboInOwl:id>
        <rdfs:label>Beza Mahafaly Reserve</rdfs:label>
    </owl:NamedIndividual>
    


    <!-- http://purl.obolibrary.org/obo/GAZ_00076527 -->

    <owl:NamedIndividual rdf:about="http://purl.obolibrary.org/obo/GAZ_00076527">
        <rdf:type rdf:resource="http://purl.obolibrary.org/obo/ENVO_00000004"/>
        <obo:RO_0001025 rdf:resource="http://purl.obolibrary.org/obo/GAZ_00032071"/>
        <obo:IAO_0000115>A district in Menabe Region, Madagascar.</obo:IAO_0000115>
        <oboInOwl:hasOBONamespace>GAZ</oboInOwl:hasOBONamespace>
        <oboInOwl:id>GAZ:00076527</oboInOwl:id>
        <rdfs:label>Miandrivazo District</rdfs:label>
    </owl:NamedIndividual>
    


    <!-- http://purl.obolibrary.org/obo/GAZ_00076528 -->

    <owl:NamedIndividual rdf:about="http://purl.obolibrary.org/obo/GAZ_00076528">
        <rdf:type rdf:resource="http://purl.obolibrary.org/obo/ENVO_00000004"/>
        <obo:RO_0001025 rdf:resource="http://purl.obolibrary.org/obo/GAZ_00032071"/>
        <obo:IAO_0000115>A district in Menabe Region, Madagascar.</obo:IAO_0000115>
        <oboInOwl:hasOBONamespace>GAZ</oboInOwl:hasOBONamespace>
        <oboInOwl:id>GAZ:00076528</oboInOwl:id>
        <rdfs:label>Mahabo District</rdfs:label>
    </owl:NamedIndividual>
    


    <!-- http://purl.obolibrary.org/obo/GAZ_00076529 -->

    <owl:NamedIndividual rdf:about="http://purl.obolibrary.org/obo/GAZ_00076529">
        <rdf:type rdf:resource="http://purl.obolibrary.org/obo/ENVO_00000004"/>
        <obo:RO_0001025 rdf:resource="http://purl.obolibrary.org/obo/GAZ_00032071"/>
        <obo:IAO_0000115>A district in Menabe Region, Madagascar.</obo:IAO_0000115>
        <oboInOwl:hasOBONamespace>GAZ</oboInOwl:hasOBONamespace>
        <oboInOwl:id>GAZ:00076529</oboInOwl:id>
        <rdfs:label>Belon&apos;i Tsiribihina District</rdfs:label>
    </owl:NamedIndividual>
    


    <!-- http://purl.obolibrary.org/obo/GAZ_00076530 -->

    <owl:NamedIndividual rdf:about="http://purl.obolibrary.org/obo/GAZ_00076530">
        <rdf:type rdf:resource="http://purl.obolibrary.org/obo/ENVO_00000004"/>
        <obo:RO_0001025 rdf:resource="http://purl.obolibrary.org/obo/GAZ_00032071"/>
        <obo:IAO_0000115>A district in Menabe Region, Madagascar.</obo:IAO_0000115>
        <oboInOwl:hasOBONamespace>GAZ</oboInOwl:hasOBONamespace>
        <oboInOwl:id>GAZ:00076530</oboInOwl:id>
        <rdfs:label>Manja District</rdfs:label>
    </owl:NamedIndividual>
    


    <!-- http://purl.obolibrary.org/obo/GAZ_00076531 -->

    <owl:NamedIndividual rdf:about="http://purl.obolibrary.org/obo/GAZ_00076531">
        <rdf:type rdf:resource="http://purl.obolibrary.org/obo/ENVO_00000004"/>
        <obo:RO_0001025 rdf:resource="http://purl.obolibrary.org/obo/GAZ_00032071"/>
        <obo:IAO_0000115>A district in Menabe Region, Madagascar.</obo:IAO_0000115>
        <oboInOwl:hasOBONamespace>GAZ</oboInOwl:hasOBONamespace>
        <oboInOwl:id>GAZ:00076531</oboInOwl:id>
        <rdfs:label>Morondava District</rdfs:label>
    </owl:NamedIndividual>
    


    <!-- http://purl.obolibrary.org/obo/GAZ_00076532 -->

    <owl:NamedIndividual rdf:about="http://purl.obolibrary.org/obo/GAZ_00076532">
        <rdf:type rdf:resource="http://purl.obolibrary.org/obo/ENVO_00000004"/>
        <obo:RO_0001025 rdf:resource="http://purl.obolibrary.org/obo/GAZ_00032068"/>
        <obo:IAO_0000115>A district in Androy Region, Madagascar.</obo:IAO_0000115>
        <oboInOwl:hasOBONamespace>GAZ</oboInOwl:hasOBONamespace>
        <oboInOwl:id>GAZ:00076532</oboInOwl:id>
        <rdfs:label>Bekily District</rdfs:label>
    </owl:NamedIndividual>
    


    <!-- http://purl.obolibrary.org/obo/GAZ_00076533 -->

    <owl:NamedIndividual rdf:about="http://purl.obolibrary.org/obo/GAZ_00076533">
        <rdf:type rdf:resource="http://purl.obolibrary.org/obo/ENVO_00000004"/>
        <obo:RO_0001025 rdf:resource="http://purl.obolibrary.org/obo/GAZ_00032068"/>
        <obo:IAO_0000115>A district in Androy Region, Madagascar.</obo:IAO_0000115>
        <oboInOwl:hasOBONamespace>GAZ</oboInOwl:hasOBONamespace>
        <oboInOwl:id>GAZ:00076533</oboInOwl:id>
        <rdfs:label>Ambovombe-Androy District</rdfs:label>
    </owl:NamedIndividual>
    


    <!-- http://purl.obolibrary.org/obo/GAZ_00076534 -->

    <owl:NamedIndividual rdf:about="http://purl.obolibrary.org/obo/GAZ_00076534">
        <rdf:type rdf:resource="http://purl.obolibrary.org/obo/ENVO_00000004"/>
        <obo:RO_0001025 rdf:resource="http://purl.obolibrary.org/obo/GAZ_00032068"/>
        <obo:IAO_0000115>A district in Androy Region, Madagascar.</obo:IAO_0000115>
        <oboInOwl:hasOBONamespace>GAZ</oboInOwl:hasOBONamespace>
        <oboInOwl:id>GAZ:00076534</oboInOwl:id>
        <rdfs:label>Beloha District</rdfs:label>
    </owl:NamedIndividual>
    


    <!-- http://purl.obolibrary.org/obo/GAZ_00076535 -->

    <owl:NamedIndividual rdf:about="http://purl.obolibrary.org/obo/GAZ_00076535">
        <rdf:type rdf:resource="http://purl.obolibrary.org/obo/ENVO_00000004"/>
        <obo:RO_0001025 rdf:resource="http://purl.obolibrary.org/obo/GAZ_00032068"/>
        <obo:IAO_0000115>A district in Androy Region, Madagascar.</obo:IAO_0000115>
        <oboInOwl:hasOBONamespace>GAZ</oboInOwl:hasOBONamespace>
        <oboInOwl:id>GAZ:00076535</oboInOwl:id>
        <rdfs:label>Tsihombe District</rdfs:label>
    </owl:NamedIndividual>
    


    <!-- http://purl.obolibrary.org/obo/GAZ_00076536 -->

    <owl:NamedIndividual rdf:about="http://purl.obolibrary.org/obo/GAZ_00076536">
        <rdf:type rdf:resource="http://purl.obolibrary.org/obo/ENVO_00000004"/>
        <obo:RO_0001025 rdf:resource="http://purl.obolibrary.org/obo/GAZ_00032057"/>
        <obo:IAO_0000115>A district in Atsimo-Atsinanana Region, Madagascar.</obo:IAO_0000115>
        <oboInOwl:hasOBONamespace>GAZ</oboInOwl:hasOBONamespace>
        <oboInOwl:id>GAZ:00076536</oboInOwl:id>
        <rdfs:label>Vondrozo District</rdfs:label>
    </owl:NamedIndividual>
    


    <!-- http://purl.obolibrary.org/obo/GAZ_00076537 -->

    <owl:NamedIndividual rdf:about="http://purl.obolibrary.org/obo/GAZ_00076537">
        <rdf:type rdf:resource="http://purl.obolibrary.org/obo/ENVO_00000004"/>
        <obo:RO_0001025 rdf:resource="http://purl.obolibrary.org/obo/GAZ_00032057"/>
        <obo:IAO_0000115>A district in Atsimo-Atsinanana Region, Madagascar.</obo:IAO_0000115>
        <oboInOwl:hasOBONamespace>GAZ</oboInOwl:hasOBONamespace>
        <oboInOwl:id>GAZ:00076537</oboInOwl:id>
        <rdfs:label>Farafangana District</rdfs:label>
    </owl:NamedIndividual>
    


    <!-- http://purl.obolibrary.org/obo/GAZ_00076538 -->

    <owl:NamedIndividual rdf:about="http://purl.obolibrary.org/obo/GAZ_00076538">
        <rdf:type rdf:resource="http://purl.obolibrary.org/obo/ENVO_00000004"/>
        <obo:RO_0001025 rdf:resource="http://purl.obolibrary.org/obo/GAZ_00032057"/>
        <obo:IAO_0000115>A district in Atsimo-Atsinanana Region, Madagascar.</obo:IAO_0000115>
        <oboInOwl:hasOBONamespace>GAZ</oboInOwl:hasOBONamespace>
        <oboInOwl:id>GAZ:00076538</oboInOwl:id>
        <rdfs:label>Befotaka District</rdfs:label>
    </owl:NamedIndividual>
    


    <!-- http://purl.obolibrary.org/obo/GAZ_00076539 -->

    <owl:NamedIndividual rdf:about="http://purl.obolibrary.org/obo/GAZ_00076539">
        <rdf:type rdf:resource="http://purl.obolibrary.org/obo/ENVO_00000004"/>
        <obo:RO_0001025 rdf:resource="http://purl.obolibrary.org/obo/GAZ_00032057"/>
        <obo:IAO_0000115>A district in Atsimo-Atsinanana Region, Madagascar.</obo:IAO_0000115>
        <oboInOwl:hasOBONamespace>GAZ</oboInOwl:hasOBONamespace>
        <oboInOwl:id>GAZ:00076539</oboInOwl:id>
        <rdfs:label>Midongy-Atsim District</rdfs:label>
    </owl:NamedIndividual>
    


    <!-- http://purl.obolibrary.org/obo/GAZ_00076540 -->

    <owl:NamedIndividual rdf:about="http://purl.obolibrary.org/obo/GAZ_00076540">
        <rdf:type rdf:resource="http://purl.obolibrary.org/obo/ENVO_00000004"/>
        <obo:RO_0001025 rdf:resource="http://purl.obolibrary.org/obo/GAZ_00032057"/>
        <obo:IAO_0000115>A district in Atsimo-Atsinanana Region, Madagascar.</obo:IAO_0000115>
        <oboInOwl:hasOBONamespace>GAZ</oboInOwl:hasOBONamespace>
        <oboInOwl:id>GAZ:00076540</oboInOwl:id>
        <rdfs:label>Vangaindrano District</rdfs:label>
    </owl:NamedIndividual>
    


    <!-- http://purl.obolibrary.org/obo/GAZ_00076541 -->

    <owl:NamedIndividual rdf:about="http://purl.obolibrary.org/obo/GAZ_00076541">
        <rdf:type rdf:resource="http://purl.obolibrary.org/obo/ENVO_00000004"/>
        <obo:RO_0001025 rdf:resource="http://purl.obolibrary.org/obo/GAZ_00032060"/>
        <obo:IAO_0000115>A district in Vatovavy Fitovinany Region, Madagascar.</obo:IAO_0000115>
        <oboInOwl:hasOBONamespace>GAZ</oboInOwl:hasOBONamespace>
        <oboInOwl:id>GAZ:00076541</oboInOwl:id>
        <rdfs:label>Mananjary District</rdfs:label>
    </owl:NamedIndividual>
    


    <!-- http://purl.obolibrary.org/obo/GAZ_00076542 -->

    <owl:NamedIndividual rdf:about="http://purl.obolibrary.org/obo/GAZ_00076542">
        <rdf:type rdf:resource="http://purl.obolibrary.org/obo/ENVO_00000004"/>
        <obo:RO_0001025 rdf:resource="http://purl.obolibrary.org/obo/GAZ_00032060"/>
        <obo:IAO_0000115>A district in Vatovavy Fitovinany Region, Madagascar.</obo:IAO_0000115>
        <oboInOwl:hasOBONamespace>GAZ</oboInOwl:hasOBONamespace>
        <oboInOwl:id>GAZ:00076542</oboInOwl:id>
        <rdfs:label>Nosy-Varika District</rdfs:label>
    </owl:NamedIndividual>
    


    <!-- http://purl.obolibrary.org/obo/GAZ_00076543 -->

    <owl:NamedIndividual rdf:about="http://purl.obolibrary.org/obo/GAZ_00076543">
        <rdf:type rdf:resource="http://purl.obolibrary.org/obo/ENVO_00000004"/>
        <obo:RO_0001025 rdf:resource="http://purl.obolibrary.org/obo/GAZ_00032060"/>
        <obo:IAO_0000115>A district in Vatovavy Fitovinany Region, Madagascar.</obo:IAO_0000115>
        <oboInOwl:hasOBONamespace>GAZ</oboInOwl:hasOBONamespace>
        <oboInOwl:id>GAZ:00076543</oboInOwl:id>
        <rdfs:label>Ifanadiana District</rdfs:label>
    </owl:NamedIndividual>
    


    <!-- http://purl.obolibrary.org/obo/GAZ_00076544 -->

    <owl:NamedIndividual rdf:about="http://purl.obolibrary.org/obo/GAZ_00076544">
        <rdf:type rdf:resource="http://purl.obolibrary.org/obo/ENVO_00000004"/>
        <obo:RO_0001025 rdf:resource="http://purl.obolibrary.org/obo/GAZ_00032060"/>
        <obo:IAO_0000115>A district in Vatovavy Fitovinany Region, Madagascar.</obo:IAO_0000115>
        <oboInOwl:hasOBONamespace>GAZ</oboInOwl:hasOBONamespace>
        <oboInOwl:id>GAZ:00076544</oboInOwl:id>
        <rdfs:label>Manakara-Atsimo District</rdfs:label>
    </owl:NamedIndividual>
    


    <!-- http://purl.obolibrary.org/obo/GAZ_00076545 -->

    <owl:NamedIndividual rdf:about="http://purl.obolibrary.org/obo/GAZ_00076545">
        <rdf:type rdf:resource="http://purl.obolibrary.org/obo/ENVO_00000004"/>
        <obo:RO_0001025 rdf:resource="http://purl.obolibrary.org/obo/GAZ_00032060"/>
        <obo:IAO_0000115>A district in Vatovavy Fitovinany Region, Madagascar.</obo:IAO_0000115>
        <oboInOwl:hasOBONamespace>GAZ</oboInOwl:hasOBONamespace>
        <oboInOwl:id>GAZ:00076545</oboInOwl:id>
        <rdfs:label>Vohipeno District</rdfs:label>
    </owl:NamedIndividual>
    


    <!-- http://purl.obolibrary.org/obo/GAZ_00076546 -->

    <owl:NamedIndividual rdf:about="http://purl.obolibrary.org/obo/GAZ_00076546">
        <rdf:type rdf:resource="http://purl.obolibrary.org/obo/ENVO_00000004"/>
        <obo:RO_0001025 rdf:resource="http://purl.obolibrary.org/obo/GAZ_00032060"/>
        <obo:IAO_0000115>A district in Vatovavy Fitovinany Region, Madagascar.</obo:IAO_0000115>
        <oboInOwl:hasOBONamespace>GAZ</oboInOwl:hasOBONamespace>
        <oboInOwl:id>GAZ:00076546</oboInOwl:id>
        <rdfs:label>Ikongo District</rdfs:label>
    </owl:NamedIndividual>
    


    <!-- http://purl.obolibrary.org/obo/GAZ_00076547 -->

    <owl:NamedIndividual rdf:about="http://purl.obolibrary.org/obo/GAZ_00076547">
        <obo:RO_0001025 rdf:resource="http://purl.obolibrary.org/obo/GAZ_00076486"/>
        <obo:IAO_0000115>A nature reserve located close to the western coast of Madagascar. A World Heritage Site.</obo:IAO_0000115>
        <oboInOwl:hasOBONamespace>GAZ</oboInOwl:hasOBONamespace>
        <oboInOwl:id>GAZ:00076547</oboInOwl:id>
        <rdfs:label>Tsingy de Bemaraha Strict Nature Reserve</rdfs:label>
    </owl:NamedIndividual>
    


    <!-- http://purl.obolibrary.org/obo/GAZ_00076548 -->

    <owl:NamedIndividual rdf:about="http://purl.obolibrary.org/obo/GAZ_00076548">
        <obo:RO_0001025 rdf:resource="http://purl.obolibrary.org/obo/GAZ_00005425"/>
        <obo:IAO_0000115>A strict nature reserve in Madagascar.</obo:IAO_0000115>
        <oboInOwl:hasOBONamespace>GAZ</oboInOwl:hasOBONamespace>
        <oboInOwl:id>GAZ:00076548</oboInOwl:id>
        <rdfs:label>Lokobe Reserve</rdfs:label>
    </owl:NamedIndividual>
    


    <!-- http://purl.obolibrary.org/obo/GAZ_00076549 -->

    <owl:NamedIndividual rdf:about="http://purl.obolibrary.org/obo/GAZ_00076549">
        <obo:RO_0001025 rdf:resource="http://purl.obolibrary.org/obo/GAZ_00005425"/>
        <obo:IAO_0000115>A strict nature reserve in Madagascar.</obo:IAO_0000115>
        <oboInOwl:hasOBONamespace>GAZ</oboInOwl:hasOBONamespace>
        <oboInOwl:id>GAZ:00076549</oboInOwl:id>
        <rdfs:label>Tsaratanana-Manongarivo Reserve</rdfs:label>
    </owl:NamedIndividual>
    


    <!-- http://purl.obolibrary.org/obo/GAZ_00076550 -->

    <owl:NamedIndividual rdf:about="http://purl.obolibrary.org/obo/GAZ_00076550">
        <obo:RO_0001025 rdf:resource="http://purl.obolibrary.org/obo/GAZ_00005423"/>
        <obo:IAO_0000115>A strict nature reserve in Madagascar.</obo:IAO_0000115>
        <oboInOwl:hasOBONamespace>GAZ</oboInOwl:hasOBONamespace>
        <oboInOwl:id>GAZ:00076550</oboInOwl:id>
        <rdfs:label>Zahamena Reserve</rdfs:label>
    </owl:NamedIndividual>
    


    <!-- http://purl.obolibrary.org/obo/GAZ_00076551 -->

    <owl:NamedIndividual rdf:about="http://purl.obolibrary.org/obo/GAZ_00076551">
        <obo:RO_0001025 rdf:resource="http://purl.obolibrary.org/obo/GAZ_00005427"/>
        <obo:IAO_0000115>A strict nature reserve in Madagascar.</obo:IAO_0000115>
        <oboInOwl:hasOBONamespace>GAZ</oboInOwl:hasOBONamespace>
        <oboInOwl:id>GAZ:00076551</oboInOwl:id>
        <rdfs:label>Betampona Reserve</rdfs:label>
    </owl:NamedIndividual>
    


    <!-- http://purl.obolibrary.org/obo/GAZ_00076552 -->

    <owl:NamedIndividual rdf:about="http://purl.obolibrary.org/obo/GAZ_00076552">
        <obo:RO_0001025 rdf:resource="http://purl.obolibrary.org/obo/GAZ_00005425"/>
        <obo:IAO_0000115>A national park in the Antsiranana Province of northern Madagascar. The park is known for its water falls and crater lakes and is located 1000 km north of the capital, Antananarivo.</obo:IAO_0000115>
        <oboInOwl:hasOBONamespace>GAZ</oboInOwl:hasOBONamespace>
        <oboInOwl:id>GAZ:00076552</oboInOwl:id>
        <rdfs:label>Amber Mountain National Park</rdfs:label>
    </owl:NamedIndividual>
    


    <!-- http://purl.obolibrary.org/obo/GAZ_00076553 -->

    <owl:NamedIndividual rdf:about="http://purl.obolibrary.org/obo/GAZ_00076553">
        <obo:RO_0001025 rdf:resource="http://purl.obolibrary.org/obo/GAZ_00001108"/>
        <oboInOwl:hasOBONamespace>GAZ</oboInOwl:hasOBONamespace>
        <oboInOwl:id>GAZ:00076553</oboInOwl:id>
        <rdfs:label>Malagasy Highlands</rdfs:label>
    </owl:NamedIndividual>
    


    <!-- http://purl.obolibrary.org/obo/GAZ_00076554 -->

    <owl:NamedIndividual rdf:about="http://purl.obolibrary.org/obo/GAZ_00076554">
        <obo:RO_0001025 rdf:resource="http://purl.obolibrary.org/obo/GAZ_00076553"/>
        <obo:IAO_0000115>The southernmost spur of the Malagasy Highlands.</obo:IAO_0000115>
        <oboInOwl:hasOBONamespace>GAZ</oboInOwl:hasOBONamespace>
        <oboInOwl:id>GAZ:00076554</oboInOwl:id>
        <rdfs:label>Anosy Mountain Range</rdfs:label>
    </owl:NamedIndividual>
    


    <!-- http://purl.obolibrary.org/obo/GAZ_00076555 -->

    <owl:NamedIndividual rdf:about="http://purl.obolibrary.org/obo/GAZ_00076555">
        <obo:RO_0001025 rdf:resource="http://purl.obolibrary.org/obo/GAZ_00076554"/>
        <obo:IAO_0000115>A national park in SE Madagascar that covers 760 km2 of the Anosy mountain range, the southernmost spur of the Malagasy Highlands.</obo:IAO_0000115>
        <oboInOwl:hasOBONamespace>GAZ</oboInOwl:hasOBONamespace>
        <oboInOwl:id>GAZ:00076555</oboInOwl:id>
        <rdfs:label>Parc national d&apos;Andohahela</rdfs:label>
    </owl:NamedIndividual>
    


    <!-- http://purl.obolibrary.org/obo/GAZ_00076556 -->

    <owl:NamedIndividual rdf:about="http://purl.obolibrary.org/obo/GAZ_00076556">
        <obo:RO_0001025 rdf:resource="http://purl.obolibrary.org/obo/GAZ_00005427"/>
        <obo:IAO_0000115>A national park in the Fianarantsoa Province of Madagascar, 47 km south of Ambalavao. Approximately 140 km of the Tropic of Capricorn crosses the park. Established in 1999.</obo:IAO_0000115>
        <oboInOwl:hasOBONamespace>GAZ</oboInOwl:hasOBONamespace>
        <oboInOwl:id>GAZ:00076556</oboInOwl:id>
        <rdfs:label>Parc national d&apos;Andringitra</rdfs:label>
    </owl:NamedIndividual>
    


    <!-- http://purl.obolibrary.org/obo/GAZ_00076557 -->

    <owl:NamedIndividual rdf:about="http://purl.obolibrary.org/obo/GAZ_00076557">
        <obo:RO_0001025 rdf:resource="http://purl.obolibrary.org/obo/GAZ_00005426"/>
        <obo:IAO_0000115>A national park in the Mahajanga Province of Madagascar. The closest city is Majunga 115 km north of the park.</obo:IAO_0000115>
        <oboInOwl:hasOBONamespace>GAZ</oboInOwl:hasOBONamespace>
        <oboInOwl:id>GAZ:00076557</oboInOwl:id>
        <rdfs:label>Ankarafantsika National Park</rdfs:label>
    </owl:NamedIndividual>
    


    <!-- http://purl.obolibrary.org/obo/GAZ_00076558 -->

    <owl:NamedIndividual rdf:about="http://purl.obolibrary.org/obo/GAZ_00076558">
        <obo:RO_0001025 rdf:resource="http://purl.obolibrary.org/obo/GAZ_00005426"/>
        <obo:IAO_0000115>A national park.</obo:IAO_0000115>
        <oboInOwl:hasOBONamespace>GAZ</oboInOwl:hasOBONamespace>
        <oboInOwl:id>GAZ:00076558</oboInOwl:id>
        <rdfs:label>Baie de Baly National Park</rdfs:label>
    </owl:NamedIndividual>
    


    <!-- http://purl.obolibrary.org/obo/GAZ_00076559 -->

    <owl:NamedIndividual rdf:about="http://purl.obolibrary.org/obo/GAZ_00076559">
        <obo:RO_0001025 rdf:resource="http://purl.obolibrary.org/obo/GAZ_00005424"/>
        <obo:IAO_0000115>A national park.</obo:IAO_0000115>
        <oboInOwl:hasOBONamespace>GAZ</oboInOwl:hasOBONamespace>
        <oboInOwl:id>GAZ:00076559</oboInOwl:id>
        <rdfs:label>Kirindy Mitea National Park</rdfs:label>
    </owl:NamedIndividual>
    


    <!-- http://purl.obolibrary.org/obo/GAZ_00076560 -->

    <owl:NamedIndividual rdf:about="http://purl.obolibrary.org/obo/GAZ_00076560">
        <obo:RO_0001025 rdf:resource="http://purl.obolibrary.org/obo/GAZ_00005425"/>
        <obo:IAO_0000115>A national park.</obo:IAO_0000115>
        <oboInOwl:hasOBONamespace>GAZ</oboInOwl:hasOBONamespace>
        <oboInOwl:id>GAZ:00076560</oboInOwl:id>
        <rdfs:label>Marojejy National Park</rdfs:label>
    </owl:NamedIndividual>
    


    <!-- http://purl.obolibrary.org/obo/GAZ_00076561 -->

    <owl:NamedIndividual rdf:about="http://purl.obolibrary.org/obo/GAZ_00076561">
        <obo:RO_0001025 rdf:resource="http://purl.obolibrary.org/obo/GAZ_00005423"/>
        <obo:IAO_0000115>The largest bay in Madagascar. It is at the northern end of the east coast of the island and for administrative purposes it is within the autonomous province of Toamasina. The bay is about 60 km long and 30 km wide, and is formed by the Masoala peninsula on its eastern side. At the northern end of the bay is the island of Nosy Mangabe and the town of Maroantsetra.</obo:IAO_0000115>
        <oboInOwl:hasOBONamespace>GAZ</oboInOwl:hasOBONamespace>
        <oboInOwl:id>GAZ:00076561</oboInOwl:id>
        <rdfs:label>Antongil Bay</rdfs:label>
    </owl:NamedIndividual>
    


    <!-- http://purl.obolibrary.org/obo/GAZ_00076562 -->

    <owl:NamedIndividual rdf:about="http://purl.obolibrary.org/obo/GAZ_00076562">
        <obo:RO_0001025 rdf:resource="http://purl.obolibrary.org/obo/GAZ_00076561"/>
        <obo:RO_0001025 rdf:resource="http://purl.obolibrary.org/obo/GAZ_00076563"/>
        <obo:IAO_0000115>A small island reserve located in Antongil Bay about 2 km offshore from the town of Maroantsetra in eastern Madagascar.</obo:IAO_0000115>
        <oboInOwl:hasOBONamespace>GAZ</oboInOwl:hasOBONamespace>
        <oboInOwl:id>GAZ:00076562</oboInOwl:id>
        <rdfs:label>Nosy Mangabe</rdfs:label>
    </owl:NamedIndividual>
    


    <!-- http://purl.obolibrary.org/obo/GAZ_00076563 -->

    <owl:NamedIndividual rdf:about="http://purl.obolibrary.org/obo/GAZ_00076563">
        <obo:RO_0001025 rdf:resource="http://purl.obolibrary.org/obo/GAZ_00005425"/>
        <obo:RO_0001025 rdf:resource="http://purl.obolibrary.org/obo/GAZ_00076564"/>
        <obo:IAO_0000115>A national park in northeast Madagascar, is the largest of the island&apos;s protected areas. Created in 1997, the park protects 2,300 km2 of rainforest and 100 km2 of marine parks.</obo:IAO_0000115>
        <oboInOwl:hasOBONamespace>GAZ</oboInOwl:hasOBONamespace>
        <oboInOwl:id>GAZ:00076563</oboInOwl:id>
        <rdfs:label>Masoala National Park</rdfs:label>
    </owl:NamedIndividual>
    


    <!-- http://purl.obolibrary.org/obo/GAZ_00076564 -->

    <owl:NamedIndividual rdf:about="http://purl.obolibrary.org/obo/GAZ_00076564">
        <obo:RO_0001025 rdf:resource="http://purl.obolibrary.org/obo/GAZ_00005423"/>
        <oboInOwl:hasOBONamespace>GAZ</oboInOwl:hasOBONamespace>
        <oboInOwl:id>GAZ:00076564</oboInOwl:id>
        <rdfs:label>Masoala Peninsula</rdfs:label>
    </owl:NamedIndividual>
    


    <!-- http://purl.obolibrary.org/obo/GAZ_00076565 -->

    <owl:NamedIndividual rdf:about="http://purl.obolibrary.org/obo/GAZ_00076565">
        <obo:RO_0001025 rdf:resource="http://purl.obolibrary.org/obo/GAZ_00005423"/>
        <obo:IAO_0000115>A national park in Madagascar.</obo:IAO_0000115>
        <oboInOwl:hasOBONamespace>GAZ</oboInOwl:hasOBONamespace>
        <oboInOwl:id>GAZ:00076565</oboInOwl:id>
        <rdfs:label>Zahamena National Park</rdfs:label>
    </owl:NamedIndividual>
    


    <!-- http://purl.obolibrary.org/obo/GAZ_00076566 -->

    <owl:NamedIndividual rdf:about="http://purl.obolibrary.org/obo/GAZ_00076566">
        <obo:RO_0001025 rdf:resource="http://purl.obolibrary.org/obo/GAZ_00005426"/>
        <obo:IAO_0000115>A national park in Madagascar.</obo:IAO_0000115>
        <oboInOwl:hasOBONamespace>GAZ</oboInOwl:hasOBONamespace>
        <oboInOwl:id>GAZ:00076566</oboInOwl:id>
        <rdfs:label>Namoroka National Park</rdfs:label>
    </owl:NamedIndividual>
    


    <!-- http://purl.obolibrary.org/obo/GAZ_00076567 -->

    <owl:NamedIndividual rdf:about="http://purl.obolibrary.org/obo/GAZ_00076567">
        <obo:RO_0001025 rdf:resource="http://purl.obolibrary.org/obo/GAZ_00005424"/>
        <obo:IAO_0000115>A national park in Madagascar.</obo:IAO_0000115>
        <oboInOwl:hasOBONamespace>GAZ</oboInOwl:hasOBONamespace>
        <oboInOwl:id>GAZ:00076567</oboInOwl:id>
        <rdfs:label>Tsimanampetsotse National Park</rdfs:label>
    </owl:NamedIndividual>
    


    <!-- http://purl.obolibrary.org/obo/GAZ_00076568 -->

    <owl:NamedIndividual rdf:about="http://purl.obolibrary.org/obo/GAZ_00076568">
        <obo:RO_0001025 rdf:resource="http://purl.obolibrary.org/obo/GAZ_00005424"/>
        <obo:IAO_0000115>A national park in Madagascar.</obo:IAO_0000115>
        <oboInOwl:hasOBONamespace>GAZ</oboInOwl:hasOBONamespace>
        <oboInOwl:id>GAZ:00076568</oboInOwl:id>
        <rdfs:label>Zombitse-Vohibasia National Park</rdfs:label>
    </owl:NamedIndividual>
    


    <!-- http://purl.obolibrary.org/obo/GAZ_00076569 -->

    <owl:NamedIndividual rdf:about="http://purl.obolibrary.org/obo/GAZ_00076569">
        <obo:RO_0001025 rdf:resource="http://purl.obolibrary.org/obo/GAZ_00005425"/>
        <obo:IAO_0000115>A small vegetated plateau in northern Madagascar with elevations that exceed 1220 m above sea level.</obo:IAO_0000115>
        <oboInOwl:hasOBONamespace>GAZ</oboInOwl:hasOBONamespace>
        <oboInOwl:id>GAZ:00076569</oboInOwl:id>
        <rdfs:label>Ankarana Reserve</rdfs:label>
    </owl:NamedIndividual>
    


    <!-- http://purl.obolibrary.org/obo/GAZ_00076570 -->

    <owl:NamedIndividual rdf:about="http://purl.obolibrary.org/obo/GAZ_00076570">
        <obo:RO_0001025 rdf:resource="http://purl.obolibrary.org/obo/GAZ_00005424"/>
        <obo:IAO_0000115>A small private reserve of gallery forest along the Mandrare river, set in the semi-arid spiny forest ecoregion of the far south of Madagascar.</obo:IAO_0000115>
        <oboInOwl:hasOBONamespace>GAZ</oboInOwl:hasOBONamespace>
        <oboInOwl:id>GAZ:00076570</oboInOwl:id>
        <rdfs:label>Berenty Reserve</rdfs:label>
    </owl:NamedIndividual>
    


    <!-- http://purl.obolibrary.org/obo/GAZ_00076571 -->

    <owl:NamedIndividual rdf:about="http://purl.obolibrary.org/obo/GAZ_00076571">
        <obo:RO_0001025 rdf:resource="http://purl.obolibrary.org/obo/GAZ_00005426"/>
        <obo:IAO_0000115>A protected area in Madagascar.</obo:IAO_0000115>
        <oboInOwl:hasOBONamespace>GAZ</oboInOwl:hasOBONamespace>
        <oboInOwl:id>GAZ:00076571</oboInOwl:id>
        <rdfs:label>Bora Reserve</rdfs:label>
    </owl:NamedIndividual>
    


    <!-- http://purl.obolibrary.org/obo/GAZ_00076572 -->

    <owl:NamedIndividual rdf:about="http://purl.obolibrary.org/obo/GAZ_00076572">
        <obo:RO_0001025 rdf:resource="http://purl.obolibrary.org/obo/GAZ_00005425"/>
        <obo:IAO_0000115>A protected area in Madagascar.</obo:IAO_0000115>
        <oboInOwl:hasOBONamespace>GAZ</oboInOwl:hasOBONamespace>
        <oboInOwl:id>GAZ:00076572</oboInOwl:id>
        <rdfs:label>Amber Forest Reserve</rdfs:label>
    </owl:NamedIndividual>
    


    <!-- http://purl.obolibrary.org/obo/GAZ_00076573 -->

    <owl:NamedIndividual rdf:about="http://purl.obolibrary.org/obo/GAZ_00076573">
        <obo:RO_0001025 rdf:resource="http://purl.obolibrary.org/obo/GAZ_00001108"/>
        <obo:IAO_0000115>A protected area in Madagascar.</obo:IAO_0000115>
        <oboInOwl:hasOBONamespace>GAZ</oboInOwl:hasOBONamespace>
        <oboInOwl:id>GAZ:00076573</oboInOwl:id>
        <rdfs:label>Anjanaharibe-Sud Reserve</rdfs:label>
    </owl:NamedIndividual>
    


    <!-- http://purl.obolibrary.org/obo/GAZ_00076574 -->

    <owl:NamedIndividual rdf:about="http://purl.obolibrary.org/obo/GAZ_00076574">
        <obo:RO_0001025 rdf:resource="http://purl.obolibrary.org/obo/GAZ_00005423"/>
        <obo:IAO_0000115>A protected area in Madagascar.</obo:IAO_0000115>
        <oboInOwl:hasOBONamespace>GAZ</oboInOwl:hasOBONamespace>
        <oboInOwl:id>GAZ:00076574</oboInOwl:id>
        <rdfs:label>Ambatovaky Reserve</rdfs:label>
    </owl:NamedIndividual>
    


    <!-- http://purl.obolibrary.org/obo/GAZ_00076575 -->

    <owl:NamedIndividual rdf:about="http://purl.obolibrary.org/obo/GAZ_00076575">
        <obo:RO_0001025 rdf:resource="http://purl.obolibrary.org/obo/GAZ_00005426"/>
        <obo:IAO_0000115>A protected area in Madagascar.</obo:IAO_0000115>
        <oboInOwl:hasOBONamespace>GAZ</oboInOwl:hasOBONamespace>
        <oboInOwl:id>GAZ:00076575</oboInOwl:id>
        <rdfs:label>Ambohijanahary Reserve</rdfs:label>
    </owl:NamedIndividual>
    


    <!-- http://purl.obolibrary.org/obo/GAZ_00076576 -->

    <owl:NamedIndividual rdf:about="http://purl.obolibrary.org/obo/GAZ_00076576">
        <obo:RO_0001025 rdf:resource="http://purl.obolibrary.org/obo/GAZ_00005424"/>
        <obo:IAO_0000115>A protected area in Madagascar.</obo:IAO_0000115>
        <oboInOwl:hasOBONamespace>GAZ</oboInOwl:hasOBONamespace>
        <oboInOwl:id>GAZ:00076576</oboInOwl:id>
        <rdfs:label>Andranomena Reserve</rdfs:label>
    </owl:NamedIndividual>
    


    <!-- http://purl.obolibrary.org/obo/GAZ_00076577 -->

    <owl:NamedIndividual rdf:about="http://purl.obolibrary.org/obo/GAZ_00076577">
        <obo:RO_0001025 rdf:resource="http://purl.obolibrary.org/obo/GAZ_00005422"/>
        <obo:IAO_0000115>A protected area in Madagascar.</obo:IAO_0000115>
        <oboInOwl:hasOBONamespace>GAZ</oboInOwl:hasOBONamespace>
        <oboInOwl:id>GAZ:00076577</oboInOwl:id>
        <rdfs:label>Ambohitantely Reserve</rdfs:label>
    </owl:NamedIndividual>
    


    <!-- http://purl.obolibrary.org/obo/GAZ_00076578 -->

    <owl:NamedIndividual rdf:about="http://purl.obolibrary.org/obo/GAZ_00076578">
        <obo:RO_0001025 rdf:resource="http://purl.obolibrary.org/obo/GAZ_00005425"/>
        <obo:IAO_0000115>A protected area in Madagascar.</obo:IAO_0000115>
        <oboInOwl:hasOBONamespace>GAZ</oboInOwl:hasOBONamespace>
        <oboInOwl:id>GAZ:00076578</oboInOwl:id>
        <rdfs:label>Analamerana Reserve</rdfs:label>
    </owl:NamedIndividual>
    


    <!-- http://purl.obolibrary.org/obo/GAZ_00076579 -->

    <owl:NamedIndividual rdf:about="http://purl.obolibrary.org/obo/GAZ_00076579">
        <obo:RO_0001025 rdf:resource="http://purl.obolibrary.org/obo/GAZ_00005427"/>
        <obo:IAO_0000115>A protected area in Madagascar.</obo:IAO_0000115>
        <oboInOwl:hasOBONamespace>GAZ</oboInOwl:hasOBONamespace>
        <oboInOwl:id>GAZ:00076579</oboInOwl:id>
        <rdfs:label>Manombo Reserve</rdfs:label>
    </owl:NamedIndividual>
    


    <!-- http://purl.obolibrary.org/obo/GAZ_00076580 -->

    <owl:NamedIndividual rdf:about="http://purl.obolibrary.org/obo/GAZ_00076580">
        <obo:RO_0001025 rdf:resource="http://purl.obolibrary.org/obo/GAZ_00005425"/>
        <obo:IAO_0000115>A protected area in Madagascar.</obo:IAO_0000115>
        <oboInOwl:hasOBONamespace>GAZ</oboInOwl:hasOBONamespace>
        <oboInOwl:id>GAZ:00076580</oboInOwl:id>
        <rdfs:label>Manongarivo Special Reserve</rdfs:label>
    </owl:NamedIndividual>
    


    <!-- http://purl.obolibrary.org/obo/GAZ_00076581 -->

    <owl:NamedIndividual rdf:about="http://purl.obolibrary.org/obo/GAZ_00076581">
        <obo:RO_0001025 rdf:resource="http://purl.obolibrary.org/obo/GAZ_00005423"/>
        <obo:IAO_0000115>A protected area in Madagascar.</obo:IAO_0000115>
        <oboInOwl:hasOBONamespace>GAZ</oboInOwl:hasOBONamespace>
        <oboInOwl:id>GAZ:00076581</oboInOwl:id>
        <rdfs:label>Analamazoatra Reserve</rdfs:label>
    </owl:NamedIndividual>
    


    <!-- http://purl.obolibrary.org/obo/GAZ_00076582 -->

    <owl:NamedIndividual rdf:about="http://purl.obolibrary.org/obo/GAZ_00076582">
        <obo:RO_0001025 rdf:resource="http://purl.obolibrary.org/obo/GAZ_00005427"/>
        <obo:IAO_0000115>A protected area in Madagascar.</obo:IAO_0000115>
        <oboInOwl:hasOBONamespace>GAZ</oboInOwl:hasOBONamespace>
        <oboInOwl:id>GAZ:00076582</oboInOwl:id>
        <rdfs:label>Pic d&apos;Ivohibe Reserve</rdfs:label>
    </owl:NamedIndividual>
    


    <!-- http://purl.obolibrary.org/obo/GAZ_00076583 -->

    <owl:NamedIndividual rdf:about="http://purl.obolibrary.org/obo/GAZ_00076583">
        <obo:RO_0001025 rdf:resource="http://purl.obolibrary.org/obo/GAZ_00005426"/>
        <obo:IAO_0000115>A protected area in Madagascar.</obo:IAO_0000115>
        <oboInOwl:hasOBONamespace>GAZ</oboInOwl:hasOBONamespace>
        <oboInOwl:id>GAZ:00076583</oboInOwl:id>
        <rdfs:label>Maningoza Reserve</rdfs:label>
    </owl:NamedIndividual>
    


    <!-- http://purl.obolibrary.org/obo/GAZ_00076584 -->

    <owl:NamedIndividual rdf:about="http://purl.obolibrary.org/obo/GAZ_00076584">
        <obo:RO_0001025 rdf:resource="http://purl.obolibrary.org/obo/GAZ_00005423"/>
        <obo:IAO_0000115>A protected area in Madagascar.</obo:IAO_0000115>
        <oboInOwl:hasOBONamespace>GAZ</oboInOwl:hasOBONamespace>
        <oboInOwl:id>GAZ:00076584</oboInOwl:id>
        <rdfs:label>Mangerivola Reserve</rdfs:label>
    </owl:NamedIndividual>
    


    <!-- http://purl.obolibrary.org/obo/GAZ_00076585 -->

    <owl:NamedIndividual rdf:about="http://purl.obolibrary.org/obo/GAZ_00076585">
        <obo:RO_0001025 rdf:resource="http://purl.obolibrary.org/obo/GAZ_00005426"/>
        <obo:IAO_0000115>A protected area in Madagascar.</obo:IAO_0000115>
        <oboInOwl:hasOBONamespace>GAZ</oboInOwl:hasOBONamespace>
        <oboInOwl:id>GAZ:00076585</oboInOwl:id>
        <rdfs:label>Kasijy Reserve</rdfs:label>
    </owl:NamedIndividual>
    


    <!-- http://purl.obolibrary.org/obo/GAZ_00076586 -->

    <owl:NamedIndividual rdf:about="http://purl.obolibrary.org/obo/GAZ_00076586">
        <obo:RO_0001025 rdf:resource="http://purl.obolibrary.org/obo/GAZ_00005426"/>
        <obo:IAO_0000115>A protected area in Madagascar.</obo:IAO_0000115>
        <oboInOwl:hasOBONamespace>GAZ</oboInOwl:hasOBONamespace>
        <oboInOwl:id>GAZ:00076586</oboInOwl:id>
        <rdfs:label>Tampoketsa Analamaitso Reserve</rdfs:label>
    </owl:NamedIndividual>
    


    <!-- http://purl.obolibrary.org/obo/GAZ_00076587 -->

    <owl:NamedIndividual rdf:about="http://purl.obolibrary.org/obo/GAZ_00076587">
        <obo:RO_0001025 rdf:resource="http://purl.obolibrary.org/obo/GAZ_00005427"/>
        <obo:IAO_0000115>A protected area in Madagascar.</obo:IAO_0000115>
        <oboInOwl:hasOBONamespace>GAZ</oboInOwl:hasOBONamespace>
        <oboInOwl:id>GAZ:00076587</oboInOwl:id>
        <rdfs:label>Kalambatritra Reserve</rdfs:label>
    </owl:NamedIndividual>
    


    <!-- http://purl.obolibrary.org/obo/GAZ_00076588 -->

    <owl:NamedIndividual rdf:about="http://purl.obolibrary.org/obo/GAZ_00076588">
        <obo:RO_0001025 rdf:resource="http://purl.obolibrary.org/obo/GAZ_00005426"/>
        <obo:IAO_0000115>A protected area in Madagascar.</obo:IAO_0000115>
        <oboInOwl:hasOBONamespace>GAZ</oboInOwl:hasOBONamespace>
        <oboInOwl:id>GAZ:00076588</oboInOwl:id>
        <rdfs:label>Marotandrano Reserve</rdfs:label>
    </owl:NamedIndividual>
    


    <!-- http://purl.obolibrary.org/obo/GAZ_00076589 -->

    <owl:NamedIndividual rdf:about="http://purl.obolibrary.org/obo/GAZ_00076589">
        <obo:RO_0001025 rdf:resource="http://purl.obolibrary.org/obo/GAZ_00005426"/>
        <obo:IAO_0000115>A protected area in Madagascar.</obo:IAO_0000115>
        <oboInOwl:hasOBONamespace>GAZ</oboInOwl:hasOBONamespace>
        <oboInOwl:id>GAZ:00076589</oboInOwl:id>
        <rdfs:label>Bemarivo Reserve</rdfs:label>
    </owl:NamedIndividual>
    


    <!-- http://purl.obolibrary.org/obo/GAZ_00076590 -->

    <owl:NamedIndividual rdf:about="http://purl.obolibrary.org/obo/GAZ_00076590">
        <obo:RO_0001025 rdf:resource="http://purl.obolibrary.org/obo/GAZ_00005424"/>
        <obo:IAO_0000115>A protected area in Madagascar.</obo:IAO_0000115>
        <oboInOwl:hasOBONamespace>GAZ</oboInOwl:hasOBONamespace>
        <oboInOwl:id>GAZ:00076590</oboInOwl:id>
        <rdfs:label>Cap Sainte Marie Reserve</rdfs:label>
    </owl:NamedIndividual>
    


    <!-- http://purl.obolibrary.org/obo/GAZ_00076591 -->

    <owl:NamedIndividual rdf:about="http://purl.obolibrary.org/obo/GAZ_00076591">
        <obo:RO_0001025 rdf:resource="http://purl.obolibrary.org/obo/GAZ_00005423"/>
        <obo:IAO_0000115>A national park in Madagascar.</obo:IAO_0000115>
        <oboInOwl:hasOBONamespace>GAZ</oboInOwl:hasOBONamespace>
        <oboInOwl:id>GAZ:00076591</oboInOwl:id>
        <rdfs:label>Mananara Nord National Park</rdfs:label>
    </owl:NamedIndividual>
    


    <!-- http://purl.obolibrary.org/obo/GAZ_00122881 -->

    <owl:NamedIndividual rdf:about="http://purl.obolibrary.org/obo/GAZ_00122881">
        <obo:RO_0001025 rdf:resource="http://purl.obolibrary.org/obo/GAZ_00076556"/>
        <obo:IAO_0000115>Un massif montagneux de Madagascar.</obo:IAO_0000115>
        <oboInOwl:hasOBONamespace>GAZ</oboInOwl:hasOBONamespace>
        <oboInOwl:id>GAZ:00122881</oboInOwl:id>
        <rdfs:label>Massif d&apos;Andringitra</rdfs:label>
    </owl:NamedIndividual>
    


    <!-- http://purl.obolibrary.org/obo/GAZ_00146615 -->

    <owl:NamedIndividual rdf:about="http://purl.obolibrary.org/obo/GAZ_00146615">
        <obo:RO_0001025 rdf:resource="http://purl.obolibrary.org/obo/GAZ_00005426"/>
        <obo:IAO_0000115>A bay on the northwestern coast of Madagascar near the city of Mahajanga, where the Betsiboka River flows into the Mozambique Channel.</obo:IAO_0000115>
        <oboInOwl:hasOBONamespace>GAZ</oboInOwl:hasOBONamespace>
        <oboInOwl:id>GAZ:00146615</oboInOwl:id>
        <rdfs:label>Bombetoka Bay</rdfs:label>
    </owl:NamedIndividual>
    


    <!-- http://purl.obolibrary.org/obo/GAZ_00146616 -->

    <owl:NamedIndividual rdf:about="http://purl.obolibrary.org/obo/GAZ_00146616">
        <obo:RO_0001025 rdf:resource="http://purl.obolibrary.org/obo/GAZ_00005425"/>
        <obo:IAO_0000115>A large natural bay along the northeast coast of Madagascar.</obo:IAO_0000115>
        <oboInOwl:hasOBONamespace>GAZ</oboInOwl:hasOBONamespace>
        <oboInOwl:id>GAZ:00146616</oboInOwl:id>
        <rdfs:label>Antsiranana Bay</rdfs:label>
    </owl:NamedIndividual>
    


    <!-- http://purl.obolibrary.org/obo/GAZ_00251841 -->

    <owl:NamedIndividual rdf:about="http://purl.obolibrary.org/obo/GAZ_00251841">
        <obo:RO_0001025 rdf:resource="http://purl.obolibrary.org/obo/GAZ_00001108"/>
        <obo:IAO_0000115>A series of man-made and natural lakes linked by rivers running down the east coast of Madagascar for about 300 miles.</obo:IAO_0000115>
        <oboInOwl:hasOBONamespace>GAZ</oboInOwl:hasOBONamespace>
        <oboInOwl:id>GAZ:00251841</oboInOwl:id>
        <rdfs:label>Canal des Pangalanes</rdfs:label>
    </owl:NamedIndividual>
    


    <!-- http://purl.obolibrary.org/obo/GAZ_00251842 -->

    <owl:NamedIndividual rdf:about="http://purl.obolibrary.org/obo/GAZ_00251842">
        <obo:RO_0001025 rdf:resource="http://purl.obolibrary.org/obo/GAZ_00076537"/>
        <obo:IAO_0000115>A city (commune urbaine) on the south-east coast of Madagascar.</obo:IAO_0000115>
        <oboInOwl:hasOBONamespace>GAZ</oboInOwl:hasOBONamespace>
        <oboInOwl:id>GAZ:00251842</oboInOwl:id>
        <rdfs:label>Farafangana</rdfs:label>
    </owl:NamedIndividual>
    


    <!-- http://purl.obolibrary.org/obo/GAZ_00251843 -->

    <owl:NamedIndividual rdf:about="http://purl.obolibrary.org/obo/GAZ_00251843">
        <obo:RO_0001025 rdf:resource="http://purl.obolibrary.org/obo/GAZ_00005423"/>
        <obo:RO_0001025 rdf:resource="http://purl.obolibrary.org/obo/GAZ_00251841"/>
        <obo:IAO_0000115>A lagoon.</obo:IAO_0000115>
        <oboInOwl:hasOBONamespace>GAZ</oboInOwl:hasOBONamespace>
        <oboInOwl:id>GAZ:00251843</oboInOwl:id>
        <rdfs:label>Lac Rasoabe</rdfs:label>
    </owl:NamedIndividual>
    


    <!-- http://purl.obolibrary.org/obo/GAZ_00251844 -->

    <owl:NamedIndividual rdf:about="http://purl.obolibrary.org/obo/GAZ_00251844">
        <obo:RO_0001025 rdf:resource="http://purl.obolibrary.org/obo/GAZ_00005423"/>
        <obo:RO_0001025 rdf:resource="http://purl.obolibrary.org/obo/GAZ_00251841"/>
        <obo:IAO_0000115>A lagoon.</obo:IAO_0000115>
        <oboInOwl:hasOBONamespace>GAZ</oboInOwl:hasOBONamespace>
        <oboInOwl:id>GAZ:00251844</oboInOwl:id>
        <rdfs:label>Lac Ampitambe-Irangy</rdfs:label>
    </owl:NamedIndividual>
    


    <!-- http://purl.obolibrary.org/obo/GAZ_00251845 -->

    <owl:NamedIndividual rdf:about="http://purl.obolibrary.org/obo/GAZ_00251845">
        <obo:RO_0001025 rdf:resource="http://purl.obolibrary.org/obo/GAZ_00005423"/>
        <obo:RO_0001025 rdf:resource="http://purl.obolibrary.org/obo/GAZ_00251841"/>
        <obo:IAO_0000115>A lagoon.</obo:IAO_0000115>
        <oboInOwl:hasOBONamespace>GAZ</oboInOwl:hasOBONamespace>
        <oboInOwl:id>GAZ:00251845</oboInOwl:id>
        <rdfs:label>Lac Rasoamasay</rdfs:label>
    </owl:NamedIndividual>
    


    <!-- http://purl.obolibrary.org/obo/GAZ_00251846 -->

    <owl:NamedIndividual rdf:about="http://purl.obolibrary.org/obo/GAZ_00251846">
        <obo:RO_0001025 rdf:resource="http://purl.obolibrary.org/obo/GAZ_00005423"/>
        <obo:RO_0001025 rdf:resource="http://purl.obolibrary.org/obo/GAZ_00251841"/>
        <obo:IAO_0000115>A lagoon.</obo:IAO_0000115>
        <oboInOwl:hasOBONamespace>GAZ</oboInOwl:hasOBONamespace>
        <oboInOwl:id>GAZ:00251846</oboInOwl:id>
        <rdfs:label>Lac Ihosy</rdfs:label>
    </owl:NamedIndividual>
    


    <!-- http://purl.obolibrary.org/obo/GAZ_00251847 -->

    <owl:NamedIndividual rdf:about="http://purl.obolibrary.org/obo/GAZ_00251847">
        <obo:RO_0001025 rdf:resource="http://purl.obolibrary.org/obo/GAZ_00251841"/>
        <obo:IAO_0000115>A lagoon.</obo:IAO_0000115>
        <oboInOwl:hasOBONamespace>GAZ</oboInOwl:hasOBONamespace>
        <oboInOwl:id>GAZ:00251847</oboInOwl:id>
        <rdfs:label>Lac Alanampolsy</rdfs:label>
    </owl:NamedIndividual>
    


    <!-- http://purl.obolibrary.org/obo/GAZ_00251848 -->

    <owl:NamedIndividual rdf:about="http://purl.obolibrary.org/obo/GAZ_00251848">
        <obo:RO_0001025 rdf:resource="http://purl.obolibrary.org/obo/GAZ_00005427"/>
        <obo:RO_0001025 rdf:resource="http://purl.obolibrary.org/obo/GAZ_00076537"/>
        <obo:RO_0001025 rdf:resource="http://purl.obolibrary.org/obo/GAZ_00251841"/>
        <obo:IAO_0000115>A lagoon.</obo:IAO_0000115>
        <oboInOwl:hasOBONamespace>GAZ</oboInOwl:hasOBONamespace>
        <oboInOwl:id>GAZ:00251848</oboInOwl:id>
        <rdfs:label>Lac Rangazavaka</rdfs:label>
    </owl:NamedIndividual>
    


    <!-- http://purl.obolibrary.org/obo/GAZ_00251849 -->

    <owl:NamedIndividual rdf:about="http://purl.obolibrary.org/obo/GAZ_00251849">
        <obo:RO_0001025 rdf:resource="http://purl.obolibrary.org/obo/GAZ_00005427"/>
        <obo:RO_0001025 rdf:resource="http://purl.obolibrary.org/obo/GAZ_00076537"/>
        <obo:RO_0001025 rdf:resource="http://purl.obolibrary.org/obo/GAZ_00251841"/>
        <obo:IAO_0000115>A lagoon.</obo:IAO_0000115>
        <oboInOwl:hasOBONamespace>GAZ</oboInOwl:hasOBONamespace>
        <oboInOwl:id>GAZ:00251849</oboInOwl:id>
        <rdfs:label>Lac Morongary</rdfs:label>
    </owl:NamedIndividual>
    


    <!-- http://purl.obolibrary.org/obo/GAZ_00251850 -->

    <owl:NamedIndividual rdf:about="http://purl.obolibrary.org/obo/GAZ_00251850">
        <obo:RO_0001025 rdf:resource="http://purl.obolibrary.org/obo/GAZ_00005427"/>
        <obo:RO_0001025 rdf:resource="http://purl.obolibrary.org/obo/GAZ_00076537"/>
        <obo:RO_0001025 rdf:resource="http://purl.obolibrary.org/obo/GAZ_00251841"/>
        <obo:IAO_0000115>A lagoon.</obo:IAO_0000115>
        <oboInOwl:hasOBONamespace>GAZ</oboInOwl:hasOBONamespace>
        <oboInOwl:id>GAZ:00251850</oboInOwl:id>
        <rdfs:label>Lac Tampolo [Fianarantsoa]</rdfs:label>
    </owl:NamedIndividual>
    


    <!-- http://purl.obolibrary.org/obo/GAZ_00251851 -->

    <owl:NamedIndividual rdf:about="http://purl.obolibrary.org/obo/GAZ_00251851">
        <obo:RO_0001025 rdf:resource="http://purl.obolibrary.org/obo/GAZ_00005423"/>
        <obo:RO_0001025 rdf:resource="http://purl.obolibrary.org/obo/GAZ_00251841"/>
        <obo:IAO_0000115>A lagoon.</obo:IAO_0000115>
        <oboInOwl:hasOBONamespace>GAZ</oboInOwl:hasOBONamespace>
        <oboInOwl:id>GAZ:00251851</oboInOwl:id>
        <rdfs:label>Lac Tampolo [Toamasina]</rdfs:label>
    </owl:NamedIndividual>
    


    <!-- http://purl.obolibrary.org/obo/GAZ_00251852 -->

    <owl:NamedIndividual rdf:about="http://purl.obolibrary.org/obo/GAZ_00251852">
        <obo:RO_0001025 rdf:resource="http://purl.obolibrary.org/obo/GAZ_00005423"/>
        <obo:IAO_0000115>A river.</obo:IAO_0000115>
        <oboInOwl:hasOBONamespace>GAZ</oboInOwl:hasOBONamespace>
        <oboInOwl:id>GAZ:00251852</oboInOwl:id>
        <rdfs:label>Ivondro River</rdfs:label>
    </owl:NamedIndividual>
    


    <!-- http://purl.obolibrary.org/obo/GAZ_00251853 -->

    <owl:NamedIndividual rdf:about="http://purl.obolibrary.org/obo/GAZ_00251853">
        <obo:RO_0001025 rdf:resource="http://purl.obolibrary.org/obo/GAZ_00005423"/>
        <obo:IAO_0000115>A river.</obo:IAO_0000115>
        <oboInOwl:hasOBONamespace>GAZ</oboInOwl:hasOBONamespace>
        <oboInOwl:id>GAZ:00251853</oboInOwl:id>
        <rdfs:label>Rianila River</rdfs:label>
    </owl:NamedIndividual>
    


    <!-- http://purl.obolibrary.org/obo/GAZ_00251854 -->

    <owl:NamedIndividual rdf:about="http://purl.obolibrary.org/obo/GAZ_00251854">
        <obo:RO_0001025 rdf:resource="http://purl.obolibrary.org/obo/GAZ_00005423"/>
        <obo:IAO_0000115>A river.</obo:IAO_0000115>
        <oboInOwl:hasOBONamespace>GAZ</oboInOwl:hasOBONamespace>
        <oboInOwl:id>GAZ:00251854</oboInOwl:id>
        <rdfs:label>Sakanila River</rdfs:label>
    </owl:NamedIndividual>
    


    <!-- http://purl.obolibrary.org/obo/GAZ_00251855 -->

    <owl:NamedIndividual rdf:about="http://purl.obolibrary.org/obo/GAZ_00251855">
        <obo:RO_0001025 rdf:resource="http://purl.obolibrary.org/obo/GAZ_00005423"/>
        <obo:IAO_0000115>A river.</obo:IAO_0000115>
        <oboInOwl:hasOBONamespace>GAZ</oboInOwl:hasOBONamespace>
        <oboInOwl:id>GAZ:00251855</oboInOwl:id>
        <rdfs:label>Mangoro River</rdfs:label>
    </owl:NamedIndividual>
    


    <!-- http://purl.obolibrary.org/obo/GAZ_00251856 -->

    <owl:NamedIndividual rdf:about="http://purl.obolibrary.org/obo/GAZ_00251856">
        <obo:RO_0001025 rdf:resource="http://purl.obolibrary.org/obo/GAZ_00005423"/>
        <obo:IAO_0000115>A river.</obo:IAO_0000115>
        <oboInOwl:hasOBONamespace>GAZ</oboInOwl:hasOBONamespace>
        <oboInOwl:id>GAZ:00251856</oboInOwl:id>
        <rdfs:label>Masora River</rdfs:label>
    </owl:NamedIndividual>
    


    <!-- http://purl.obolibrary.org/obo/GAZ_00251857 -->

    <owl:NamedIndividual rdf:about="http://purl.obolibrary.org/obo/GAZ_00251857">
        <obo:RO_0001025 rdf:resource="http://purl.obolibrary.org/obo/GAZ_00076537"/>
        <obo:IAO_0000115>A river.</obo:IAO_0000115>
        <oboInOwl:hasOBONamespace>GAZ</oboInOwl:hasOBONamespace>
        <oboInOwl:id>GAZ:00251857</oboInOwl:id>
        <rdfs:label>Mananjary River</rdfs:label>
    </owl:NamedIndividual>
    


    <!-- http://purl.obolibrary.org/obo/GAZ_00251858 -->

    <owl:NamedIndividual rdf:about="http://purl.obolibrary.org/obo/GAZ_00251858">
        <obo:RO_0001025 rdf:resource="http://purl.obolibrary.org/obo/GAZ_00076537"/>
        <obo:IAO_0000115>A river.</obo:IAO_0000115>
        <oboInOwl:hasOBONamespace>GAZ</oboInOwl:hasOBONamespace>
        <oboInOwl:id>GAZ:00251858</oboInOwl:id>
        <rdfs:label>Faraony River</rdfs:label>
    </owl:NamedIndividual>
    


    <!-- http://purl.obolibrary.org/obo/GAZ_00251859 -->

    <owl:NamedIndividual rdf:about="http://purl.obolibrary.org/obo/GAZ_00251859">
        <obo:RO_0001025 rdf:resource="http://purl.obolibrary.org/obo/GAZ_00076537"/>
        <obo:IAO_0000115>A river.</obo:IAO_0000115>
        <oboInOwl:hasOBONamespace>GAZ</oboInOwl:hasOBONamespace>
        <oboInOwl:id>GAZ:00251859</oboInOwl:id>
        <rdfs:label>Matitanana River</rdfs:label>
    </owl:NamedIndividual>
    


    <!-- http://purl.obolibrary.org/obo/GAZ_00251860 -->

    <owl:NamedIndividual rdf:about="http://purl.obolibrary.org/obo/GAZ_00251860">
        <obo:RO_0001025 rdf:resource="http://purl.obolibrary.org/obo/GAZ_00076537"/>
        <obo:IAO_0000115>A river.</obo:IAO_0000115>
        <oboInOwl:hasOBONamespace>GAZ</oboInOwl:hasOBONamespace>
        <oboInOwl:id>GAZ:00251860</oboInOwl:id>
        <rdfs:label>Manampatrana River</rdfs:label>
    </owl:NamedIndividual>
    


    <!-- http://purl.obolibrary.org/obo/GAZ_00251861 -->

    <owl:NamedIndividual rdf:about="http://purl.obolibrary.org/obo/GAZ_00251861">
        <obo:RO_0001025 rdf:resource="http://purl.obolibrary.org/obo/GAZ_00005426"/>
        <obo:IAO_0000115>A lagoon.</obo:IAO_0000115>
        <oboInOwl:hasOBONamespace>GAZ</oboInOwl:hasOBONamespace>
        <oboInOwl:id>GAZ:00251861</oboInOwl:id>
        <rdfs:label>Loza Lagoon</rdfs:label>
    </owl:NamedIndividual>
    


    <!-- http://purl.obolibrary.org/obo/GAZ_00251864 -->

    <owl:NamedIndividual rdf:about="http://purl.obolibrary.org/obo/GAZ_00251864">
        <obo:RO_0001025 rdf:resource="http://purl.obolibrary.org/obo/GAZ_00076516"/>
        <obo:IAO_0000115>A complex of lagoons.</obo:IAO_0000115>
        <oboInOwl:hasOBONamespace>GAZ</oboInOwl:hasOBONamespace>
        <oboInOwl:id>GAZ:00251864</oboInOwl:id>
        <rdfs:label>Tolanaro Lagoon Complex</rdfs:label>
    </owl:NamedIndividual>
    


    <!-- http://purl.obolibrary.org/obo/GAZ_00251865 -->

    <owl:NamedIndividual rdf:about="http://purl.obolibrary.org/obo/GAZ_00251865">
        <obo:RO_0001025 rdf:resource="http://purl.obolibrary.org/obo/GAZ_00251864"/>
        <obo:IAO_0000115>A lagoon.</obo:IAO_0000115>
        <oboInOwl:hasOBONamespace>GAZ</oboInOwl:hasOBONamespace>
        <oboInOwl:id>GAZ:00251865</oboInOwl:id>
        <rdfs:label>Lac Anony</rdfs:label>
    </owl:NamedIndividual>
    


    <!-- http://purl.obolibrary.org/obo/GAZ_00251866 -->

    <owl:NamedIndividual rdf:about="http://purl.obolibrary.org/obo/GAZ_00251866">
        <obo:RO_0001025 rdf:resource="http://purl.obolibrary.org/obo/GAZ_00251864"/>
        <obo:IAO_0000115>A lagoon.</obo:IAO_0000115>
        <oboInOwl:hasOBONamespace>GAZ</oboInOwl:hasOBONamespace>
        <oboInOwl:id>GAZ:00251866</oboInOwl:id>
        <rdfs:label>Lac Mananivo</rdfs:label>
    </owl:NamedIndividual>
    


    <!-- http://purl.obolibrary.org/obo/GAZ_00251867 -->

    <owl:NamedIndividual rdf:about="http://purl.obolibrary.org/obo/GAZ_00251867">
        <obo:RO_0001025 rdf:resource="http://purl.obolibrary.org/obo/GAZ_00251864"/>
        <obo:IAO_0000115>A lagoon.</obo:IAO_0000115>
        <oboInOwl:hasOBONamespace>GAZ</oboInOwl:hasOBONamespace>
        <oboInOwl:id>GAZ:00251867</oboInOwl:id>
        <rdfs:label>Lac Ambavarano</rdfs:label>
    </owl:NamedIndividual>
    


    <!-- http://purl.obolibrary.org/obo/GAZ_00251868 -->

    <owl:NamedIndividual rdf:about="http://purl.obolibrary.org/obo/GAZ_00251868">
        <obo:RO_0001025 rdf:resource="http://purl.obolibrary.org/obo/GAZ_00251864"/>
        <obo:IAO_0000115>A lagoon.</obo:IAO_0000115>
        <oboInOwl:hasOBONamespace>GAZ</oboInOwl:hasOBONamespace>
        <oboInOwl:id>GAZ:00251868</oboInOwl:id>
        <rdfs:label>Lac Lanirano</rdfs:label>
    </owl:NamedIndividual>
    


    <!-- http://purl.obolibrary.org/obo/GAZ_00251869 -->

    <owl:NamedIndividual rdf:about="http://purl.obolibrary.org/obo/GAZ_00251869">
        <obo:RO_0001025 rdf:resource="http://purl.obolibrary.org/obo/GAZ_00251864"/>
        <obo:IAO_0000115>A lagoon.</obo:IAO_0000115>
        <oboInOwl:hasOBONamespace>GAZ</oboInOwl:hasOBONamespace>
        <oboInOwl:id>GAZ:00251869</oboInOwl:id>
        <rdfs:label>Lac Andriambe</rdfs:label>
    </owl:NamedIndividual>
    


    <!-- http://purl.obolibrary.org/obo/GAZ_00251870 -->

    <owl:NamedIndividual rdf:about="http://purl.obolibrary.org/obo/GAZ_00251870">
        <obo:RO_0001025 rdf:resource="http://purl.obolibrary.org/obo/GAZ_00251864"/>
        <obo:IAO_0000115>A lagoon.</obo:IAO_0000115>
        <oboInOwl:hasOBONamespace>GAZ</oboInOwl:hasOBONamespace>
        <oboInOwl:id>GAZ:00251870</oboInOwl:id>
        <rdfs:label>Lac Andranasy</rdfs:label>
    </owl:NamedIndividual>
    


    <!-- http://purl.obolibrary.org/obo/GAZ_00251871 -->

    <owl:NamedIndividual rdf:about="http://purl.obolibrary.org/obo/GAZ_00251871">
        <obo:RO_0001025 rdf:resource="http://purl.obolibrary.org/obo/GAZ_00251864"/>
        <obo:IAO_0000115>A lagoon.</obo:IAO_0000115>
        <oboInOwl:hasOBONamespace>GAZ</oboInOwl:hasOBONamespace>
        <oboInOwl:id>GAZ:00251871</oboInOwl:id>
        <rdfs:label>Lac Andratoloharano</rdfs:label>
    </owl:NamedIndividual>
    


    <!-- http://purl.obolibrary.org/obo/GAZ_00251872 -->

    <owl:NamedIndividual rdf:about="http://purl.obolibrary.org/obo/GAZ_00251872">
        <obo:RO_0001025 rdf:resource="http://purl.obolibrary.org/obo/GAZ_00251864"/>
        <obo:IAO_0000115>A lagoon.</obo:IAO_0000115>
        <oboInOwl:hasOBONamespace>GAZ</oboInOwl:hasOBONamespace>
        <oboInOwl:id>GAZ:00251872</oboInOwl:id>
        <rdfs:label>Lac Ranofotsy</rdfs:label>
    </owl:NamedIndividual>
    


    <!-- http://purl.obolibrary.org/obo/GAZ_00251873 -->

    <owl:NamedIndividual rdf:about="http://purl.obolibrary.org/obo/GAZ_00251873">
        <obo:RO_0001025 rdf:resource="http://purl.obolibrary.org/obo/GAZ_00005425"/>
        <obo:IAO_0000115>A coastal lagoon.</obo:IAO_0000115>
        <oboInOwl:hasOBONamespace>GAZ</oboInOwl:hasOBONamespace>
        <oboInOwl:id>GAZ:00251873</oboInOwl:id>
        <rdfs:label>Lac Ampahana</rdfs:label>
    </owl:NamedIndividual>
    


    <!-- http://purl.obolibrary.org/obo/GAZ_00251874 -->

    <owl:NamedIndividual rdf:about="http://purl.obolibrary.org/obo/GAZ_00251874">
        <obo:RO_0001025 rdf:resource="http://purl.obolibrary.org/obo/GAZ_00005426"/>
        <obo:IAO_0000115>A river. It originates near Falaise de l&apos;Angavo. It discharges to the Indian Ocean at Bombetoka Bay.</obo:IAO_0000115>
        <oboInOwl:hasOBONamespace>GAZ</oboInOwl:hasOBONamespace>
        <oboInOwl:id>GAZ:00251874</oboInOwl:id>
        <rdfs:label>Betsiboka</rdfs:label>
    </owl:NamedIndividual>
    


    <!-- http://purl.obolibrary.org/obo/GAZ_00251878 -->

    <owl:NamedIndividual rdf:about="http://purl.obolibrary.org/obo/GAZ_00251878">
        <obo:RO_0001025 rdf:resource="http://purl.obolibrary.org/obo/GAZ_00005426"/>
        <obo:IAO_0000115>A lake. Located on the floodplain of the Betsiboka River.</obo:IAO_0000115>
        <oboInOwl:hasOBONamespace>GAZ</oboInOwl:hasOBONamespace>
        <oboInOwl:id>GAZ:00251878</oboInOwl:id>
        <rdfs:label>Lac Amparihibe</rdfs:label>
    </owl:NamedIndividual>
    


    <!-- http://purl.obolibrary.org/obo/GAZ_00251879 -->

    <owl:NamedIndividual rdf:about="http://purl.obolibrary.org/obo/GAZ_00251879">
        <obo:RO_0001025 rdf:resource="http://purl.obolibrary.org/obo/GAZ_00005426"/>
        <obo:IAO_0000115>A lake. Located on the floodplain of the Betsiboka River.</obo:IAO_0000115>
        <oboInOwl:hasOBONamespace>GAZ</oboInOwl:hasOBONamespace>
        <oboInOwl:id>GAZ:00251879</oboInOwl:id>
        <rdfs:label>Lac Ambania</rdfs:label>
    </owl:NamedIndividual>
    


    <!-- http://purl.obolibrary.org/obo/GAZ_00251880 -->

    <owl:NamedIndividual rdf:about="http://purl.obolibrary.org/obo/GAZ_00251880">
        <obo:RO_0001025 rdf:resource="http://purl.obolibrary.org/obo/GAZ_00005426"/>
        <obo:IAO_0000115>A lake. Located on the floodplain of the Betsiboka River.</obo:IAO_0000115>
        <oboInOwl:hasOBONamespace>GAZ</oboInOwl:hasOBONamespace>
        <oboInOwl:id>GAZ:00251880</oboInOwl:id>
        <rdfs:label>Lac Amboromalandy</rdfs:label>
    </owl:NamedIndividual>
    


    <!-- http://purl.obolibrary.org/obo/GAZ_00251881 -->

    <owl:NamedIndividual rdf:about="http://purl.obolibrary.org/obo/GAZ_00251881">
        <obo:RO_0001025 rdf:resource="http://purl.obolibrary.org/obo/GAZ_00005426"/>
        <obo:IAO_0000115>A lake. Located on the floodplain of the Betsiboka River.</obo:IAO_0000115>
        <oboInOwl:hasOBONamespace>GAZ</oboInOwl:hasOBONamespace>
        <oboInOwl:id>GAZ:00251881</oboInOwl:id>
        <rdfs:label>Lac Bendrony</rdfs:label>
    </owl:NamedIndividual>
    


    <!-- http://purl.obolibrary.org/obo/GAZ_00251882 -->

    <owl:NamedIndividual rdf:about="http://purl.obolibrary.org/obo/GAZ_00251882">
        <obo:RO_0001025 rdf:resource="http://purl.obolibrary.org/obo/GAZ_00005426"/>
        <obo:IAO_0000115>A lake. Located on the floodplain of the Betsiboka River.</obo:IAO_0000115>
        <oboInOwl:hasOBONamespace>GAZ</oboInOwl:hasOBONamespace>
        <oboInOwl:id>GAZ:00251882</oboInOwl:id>
        <rdfs:label>Lac Matsiabe</rdfs:label>
    </owl:NamedIndividual>
    


    <!-- 
    ///////////////////////////////////////////////////////////////////////////////////////
    //
    // Annotations
    //
    ///////////////////////////////////////////////////////////////////////////////////////
     -->

    <rdf:Description rdf:about="http://purl.obolibrary.org/obo/GAZ_00005421">
        <oboInOwl:hasOBONamespace>GAZ</oboInOwl:hasOBONamespace>
        <rdfs:label>Province (Madagascar)</rdfs:label>
        <oboInOwl:id>GAZ:00005421</oboInOwl:id>
    </rdf:Description>
    <rdf:Description rdf:about="http://purl.obolibrary.org/obo/GAZ_00005422">
        <oboInOwl:hasOBONamespace>GAZ</oboInOwl:hasOBONamespace>
        <rdfs:label>Antananarivo Province</rdfs:label>
        <obo:IAO_0000115>A province of Madagascar.</obo:IAO_0000115>
        <oboInOwl:id>GAZ:00005422</oboInOwl:id>
    </rdf:Description>
    <rdf:Description rdf:about="http://purl.obolibrary.org/obo/GAZ_00005423">
        <oboInOwl:hasOBONamespace>GAZ</oboInOwl:hasOBONamespace>
        <rdfs:label>Toamasina Province</rdfs:label>
        <oboInOwl:id>GAZ:00005423</oboInOwl:id>
        <obo:IAO_0000115>A province of Madagascar.</obo:IAO_0000115>
    </rdf:Description>
    <rdf:Description rdf:about="http://purl.obolibrary.org/obo/GAZ_00005424">
        <oboInOwl:id>GAZ:00005424</oboInOwl:id>
        <rdfs:label>Toliara Province</rdfs:label>
        <obo:IAO_0000115>A province of Madagascar.</obo:IAO_0000115>
        <oboInOwl:hasOBONamespace>GAZ</oboInOwl:hasOBONamespace>
    </rdf:Description>
    <rdf:Description rdf:about="http://purl.obolibrary.org/obo/GAZ_00005425">
        <rdfs:label>Antsiranana Province</rdfs:label>
        <oboInOwl:id>GAZ:00005425</oboInOwl:id>
        <oboInOwl:hasOBONamespace>GAZ</oboInOwl:hasOBONamespace>
        <obo:IAO_0000115>A province of Madagascar.</obo:IAO_0000115>
    </rdf:Description>
    <rdf:Description rdf:about="http://purl.obolibrary.org/obo/GAZ_00005426">
        <rdfs:label>Mahajanga Province</rdfs:label>
        <oboInOwl:id>GAZ:00005426</oboInOwl:id>
        <obo:IAO_0000115>A province of Madagascar.</obo:IAO_0000115>
        <oboInOwl:hasOBONamespace>GAZ</oboInOwl:hasOBONamespace>
    </rdf:Description>
    <rdf:Description rdf:about="http://purl.obolibrary.org/obo/GAZ_00005427">
        <obo:IAO_0000115>A province of Madagascar. The province is home to four major national parks: Ranomafana National Park, Midongy Du Sud, Isalo National Park, and Andringitra.</obo:IAO_0000115>
        <oboInOwl:id>GAZ:00005427</oboInOwl:id>
        <rdfs:label>Fianarantsoa Province</rdfs:label>
        <oboInOwl:hasOBONamespace>GAZ</oboInOwl:hasOBONamespace>
    </rdf:Description>
    <rdf:Description rdf:about="http://purl.obolibrary.org/obo/GAZ_00005432">
        <rdfs:label>populated place, Madagascar</rdfs:label>
        <oboInOwl:id>GAZ:00005432</oboInOwl:id>
        <oboInOwl:hasOBONamespace>GAZ</oboInOwl:hasOBONamespace>
    </rdf:Description>
    <rdf:Description rdf:about="http://purl.obolibrary.org/obo/GAZ_00005433">
        <oboInOwl:id>GAZ:00005433</oboInOwl:id>
        <obo:IAO_0000115>A city (commune urbaine). The capital of the Atsinanana region and of the Toamasina Province.</obo:IAO_0000115>
        <oboInOwl:hasOBONamespace>GAZ</oboInOwl:hasOBONamespace>
        <rdfs:label>Toamasina</rdfs:label>
    </rdf:Description>
    <rdf:Description rdf:about="http://purl.obolibrary.org/obo/GAZ_00008593">
        <obo:IAO_0000115>A populated place. A town in Toliara Province, Madagascar.</obo:IAO_0000115>
        <oboInOwl:id>GAZ:00008593</oboInOwl:id>
        <oboInOwl:hasOBONamespace>GAZ</oboInOwl:hasOBONamespace>
        <rdfs:label>Bekily</rdfs:label>
    </rdf:Description>
    <rdf:Description rdf:about="http://purl.obolibrary.org/obo/GAZ_00010058">
        <oboInOwl:hasOBONamespace>GAZ</oboInOwl:hasOBONamespace>
        <oboInOwl:id>GAZ:00010058</oboInOwl:id>
        <rdfs:label>Mahajanga</rdfs:label>
        <obo:IAO_0000115>A city on the north-west coast of Madagascar.</obo:IAO_0000115>
    </rdf:Description>
</rdf:RDF>



<!-- Generated by the OWL API (version 4.5.6) https://github.com/owlcs/owlapi -->

