<?xml version="1.0"?>
<rdf:RDF xmlns="http://purl.obolibrary.org/obo/gaz/subsets/countries/Mongolia.owl#"
     xml:base="http://purl.obolibrary.org/obo/gaz/subsets/countries/Mongolia.owl"
     xmlns:obo="http://purl.obolibrary.org/obo/"
     xmlns:owl="http://www.w3.org/2002/07/owl#"
     xmlns:rdf="http://www.w3.org/1999/02/22-rdf-syntax-ns#"
     xmlns:xml="http://www.w3.org/XML/1998/namespace"
     xmlns:xsd="http://www.w3.org/2001/XMLSchema#"
     xmlns:rdfs="http://www.w3.org/2000/01/rdf-schema#"
     xmlns:oboInOwl="http://www.geneontology.org/formats/oboInOwl#">
    <owl:Ontology rdf:about="http://purl.obolibrary.org/obo/gaz/subsets/countries/Mongolia.owl">
        <owl:imports rdf:resource="http://purl.obolibrary.org/obo/gaz/imports/envo_import.owl"/>
        <owl:imports rdf:resource="http://purl.obolibrary.org/obo/gaz/imports/ro_import.owl"/>
    </owl:Ontology>
    


    <!-- 
    ///////////////////////////////////////////////////////////////////////////////////////
    //
    // Annotation properties
    //
    ///////////////////////////////////////////////////////////////////////////////////////
     -->

    


    <!-- http://purl.obolibrary.org/obo/IAO_0000115 -->

    <owl:AnnotationProperty rdf:about="http://purl.obolibrary.org/obo/IAO_0000115"/>
    


    <!-- http://www.geneontology.org/formats/oboInOwl#hasOBONamespace -->

    <owl:AnnotationProperty rdf:about="http://www.geneontology.org/formats/oboInOwl#hasOBONamespace"/>
    


    <!-- http://www.geneontology.org/formats/oboInOwl#id -->

    <owl:AnnotationProperty rdf:about="http://www.geneontology.org/formats/oboInOwl#id"/>
    


    <!-- 
    ///////////////////////////////////////////////////////////////////////////////////////
    //
    // Object Properties
    //
    ///////////////////////////////////////////////////////////////////////////////////////
     -->

    


    <!-- http://purl.obolibrary.org/obo/RO_0001025 -->

    <owl:ObjectProperty rdf:about="http://purl.obolibrary.org/obo/RO_0001025"/>
    


    <!-- 
    ///////////////////////////////////////////////////////////////////////////////////////
    //
    // Classes
    //
    ///////////////////////////////////////////////////////////////////////////////////////
     -->

    


    <!-- http://purl.obolibrary.org/obo/ENVO_00000004 -->

    <owl:Class rdf:about="http://purl.obolibrary.org/obo/ENVO_00000004"/>
    


    <!-- http://purl.obolibrary.org/obo/ENVO_00000009 -->

    <owl:Class rdf:about="http://purl.obolibrary.org/obo/ENVO_00000009"/>
    


    <!-- http://purl.obolibrary.org/obo/ENVO_00000100 -->

    <owl:Class rdf:about="http://purl.obolibrary.org/obo/ENVO_00000100"/>
    


    <!-- http://purl.obolibrary.org/obo/ENVO_00000106 -->

    <owl:Class rdf:about="http://purl.obolibrary.org/obo/ENVO_00000106"/>
    


    <!-- http://purl.obolibrary.org/obo/ENVO_00000275 -->

    <owl:Class rdf:about="http://purl.obolibrary.org/obo/ENVO_00000275"/>
    


    <!-- http://purl.obolibrary.org/obo/ENVO_00000856 -->

    <owl:Class rdf:about="http://purl.obolibrary.org/obo/ENVO_00000856"/>
    


    <!-- http://purl.obolibrary.org/obo/GAZ_00009465 -->

    <owl:Class rdf:about="http://purl.obolibrary.org/obo/GAZ_00009465"/>
    


    <!-- http://purl.obolibrary.org/obo/GAZ_00014867 -->

    <owl:Class rdf:about="http://purl.obolibrary.org/obo/GAZ_00014867">
        <rdfs:subClassOf rdf:resource="http://purl.obolibrary.org/obo/GAZ_00009465"/>
    </owl:Class>
    


    <!-- http://purl.obolibrary.org/obo/GAZ_00014868 -->

    <owl:Class rdf:about="http://purl.obolibrary.org/obo/GAZ_00014868">
        <rdfs:subClassOf rdf:resource="http://purl.obolibrary.org/obo/GAZ_00009465"/>
    </owl:Class>
    


    <!-- http://purl.obolibrary.org/obo/GAZ_00014869 -->

    <owl:Class rdf:about="http://purl.obolibrary.org/obo/GAZ_00014869">
        <rdfs:subClassOf rdf:resource="http://purl.obolibrary.org/obo/GAZ_00009465"/>
    </owl:Class>
    


    <!-- http://purl.obolibrary.org/obo/GAZ_00014870 -->

    <owl:Class rdf:about="http://purl.obolibrary.org/obo/GAZ_00014870">
        <rdfs:subClassOf rdf:resource="http://purl.obolibrary.org/obo/GAZ_00009465"/>
    </owl:Class>
    


    <!-- http://purl.obolibrary.org/obo/GAZ_00014871 -->

    <owl:Class rdf:about="http://purl.obolibrary.org/obo/GAZ_00014871">
        <rdfs:subClassOf rdf:resource="http://purl.obolibrary.org/obo/GAZ_00009465"/>
    </owl:Class>
    


    <!-- http://purl.obolibrary.org/obo/GAZ_00014872 -->

    <owl:Class rdf:about="http://purl.obolibrary.org/obo/GAZ_00014872">
        <rdfs:subClassOf rdf:resource="http://purl.obolibrary.org/obo/GAZ_00009465"/>
    </owl:Class>
    


    <!-- http://purl.obolibrary.org/obo/GAZ_00014873 -->

    <owl:Class rdf:about="http://purl.obolibrary.org/obo/GAZ_00014873">
        <rdfs:subClassOf rdf:resource="http://purl.obolibrary.org/obo/GAZ_00009465"/>
    </owl:Class>
    


    <!-- http://purl.obolibrary.org/obo/GAZ_00014874 -->

    <owl:Class rdf:about="http://purl.obolibrary.org/obo/GAZ_00014874">
        <rdfs:subClassOf rdf:resource="http://purl.obolibrary.org/obo/GAZ_00009465"/>
    </owl:Class>
    


    <!-- http://purl.obolibrary.org/obo/GAZ_00014875 -->

    <owl:Class rdf:about="http://purl.obolibrary.org/obo/GAZ_00014875">
        <rdfs:subClassOf rdf:resource="http://purl.obolibrary.org/obo/GAZ_00009465"/>
    </owl:Class>
    


    <!-- http://purl.obolibrary.org/obo/GAZ_00014876 -->

    <owl:Class rdf:about="http://purl.obolibrary.org/obo/GAZ_00014876">
        <rdfs:subClassOf rdf:resource="http://purl.obolibrary.org/obo/GAZ_00009465"/>
    </owl:Class>
    


    <!-- http://purl.obolibrary.org/obo/GAZ_00014877 -->

    <owl:Class rdf:about="http://purl.obolibrary.org/obo/GAZ_00014877">
        <rdfs:subClassOf rdf:resource="http://purl.obolibrary.org/obo/GAZ_00009465"/>
    </owl:Class>
    


    <!-- http://purl.obolibrary.org/obo/GAZ_00014878 -->

    <owl:Class rdf:about="http://purl.obolibrary.org/obo/GAZ_00014878">
        <rdfs:subClassOf rdf:resource="http://purl.obolibrary.org/obo/GAZ_00009465"/>
    </owl:Class>
    


    <!-- http://purl.obolibrary.org/obo/GAZ_00014879 -->

    <owl:Class rdf:about="http://purl.obolibrary.org/obo/GAZ_00014879">
        <rdfs:subClassOf rdf:resource="http://purl.obolibrary.org/obo/GAZ_00009465"/>
    </owl:Class>
    


    <!-- http://purl.obolibrary.org/obo/GAZ_00014880 -->

    <owl:Class rdf:about="http://purl.obolibrary.org/obo/GAZ_00014880">
        <rdfs:subClassOf rdf:resource="http://purl.obolibrary.org/obo/GAZ_00009465"/>
    </owl:Class>
    


    <!-- http://purl.obolibrary.org/obo/GAZ_00014881 -->

    <owl:Class rdf:about="http://purl.obolibrary.org/obo/GAZ_00014881">
        <rdfs:subClassOf rdf:resource="http://purl.obolibrary.org/obo/GAZ_00009465"/>
    </owl:Class>
    


    <!-- http://purl.obolibrary.org/obo/GAZ_00014882 -->

    <owl:Class rdf:about="http://purl.obolibrary.org/obo/GAZ_00014882">
        <rdfs:subClassOf rdf:resource="http://purl.obolibrary.org/obo/GAZ_00009465"/>
    </owl:Class>
    


    <!-- http://purl.obolibrary.org/obo/GAZ_00014883 -->

    <owl:Class rdf:about="http://purl.obolibrary.org/obo/GAZ_00014883">
        <rdfs:subClassOf rdf:resource="http://purl.obolibrary.org/obo/GAZ_00009465"/>
    </owl:Class>
    


    <!-- http://purl.obolibrary.org/obo/GAZ_00014884 -->

    <owl:Class rdf:about="http://purl.obolibrary.org/obo/GAZ_00014884">
        <rdfs:subClassOf rdf:resource="http://purl.obolibrary.org/obo/GAZ_00009465"/>
    </owl:Class>
    


    <!-- http://purl.obolibrary.org/obo/GAZ_00014885 -->

    <owl:Class rdf:about="http://purl.obolibrary.org/obo/GAZ_00014885">
        <rdfs:subClassOf rdf:resource="http://purl.obolibrary.org/obo/GAZ_00009465"/>
    </owl:Class>
    


    <!-- http://purl.obolibrary.org/obo/GAZ_00014886 -->

    <owl:Class rdf:about="http://purl.obolibrary.org/obo/GAZ_00014886">
        <rdfs:subClassOf rdf:resource="http://purl.obolibrary.org/obo/GAZ_00009465"/>
    </owl:Class>
    


    <!-- http://purl.obolibrary.org/obo/GAZ_00014887 -->

    <owl:Class rdf:about="http://purl.obolibrary.org/obo/GAZ_00014887">
        <rdfs:subClassOf rdf:resource="http://purl.obolibrary.org/obo/GAZ_00009465"/>
    </owl:Class>
    


    <!-- http://purl.obolibrary.org/obo/GAZ_00252209 -->

    <owl:Class rdf:about="http://purl.obolibrary.org/obo/GAZ_00252209"/>
    


    <!-- 
    ///////////////////////////////////////////////////////////////////////////////////////
    //
    // Individuals
    //
    ///////////////////////////////////////////////////////////////////////////////////////
     -->

    


    <!-- http://purl.obolibrary.org/obo/GAZ_00008744 -->

    <owl:NamedIndividual rdf:about="http://purl.obolibrary.org/obo/GAZ_00008744">
        <rdf:type rdf:resource="http://purl.obolibrary.org/obo/ENVO_00000009"/>
        <obo:IAO_0000115>A country in East-Central Asia. The landlocked country borders Russia to the north and China to the south. The capital and largest city is Ulan Bator. Mongolia is divided into 21 aimags (provinces), which are in turn divided into 315 sums (districts). The capital Ulan Bator is administrated separately as a khot (municipality) with provincial status.</obo:IAO_0000115>
        <oboInOwl:hasOBONamespace>GAZ</oboInOwl:hasOBONamespace>
        <oboInOwl:id>GAZ:00008744</oboInOwl:id>
        <rdfs:label>Mongolia</rdfs:label>
    </owl:NamedIndividual>
    


    <!-- http://purl.obolibrary.org/obo/GAZ_00008745 -->

    <owl:NamedIndividual rdf:about="http://purl.obolibrary.org/obo/GAZ_00008745">
        <obo:RO_0001025 rdf:resource="http://purl.obolibrary.org/obo/GAZ_00008744"/>
        <obo:IAO_0000115>A saline lake.</obo:IAO_0000115>
        <oboInOwl:hasOBONamespace>GAZ</oboInOwl:hasOBONamespace>
        <oboInOwl:id>GAZ:00008745</oboInOwl:id>
        <rdfs:label>Khotontyn Nuur</rdfs:label>
    </owl:NamedIndividual>
    


    <!-- http://purl.obolibrary.org/obo/GAZ_00009465 -->

    <owl:NamedIndividual rdf:about="http://purl.obolibrary.org/obo/GAZ_00009465">
        <obo:RO_0001025 rdf:resource="http://purl.obolibrary.org/obo/GAZ_00008744"/>
    </owl:NamedIndividual>
    


    <!-- http://purl.obolibrary.org/obo/GAZ_00014867 -->

    <owl:NamedIndividual rdf:about="http://purl.obolibrary.org/obo/GAZ_00014867"/>
    


    <!-- http://purl.obolibrary.org/obo/GAZ_00014868 -->

    <owl:NamedIndividual rdf:about="http://purl.obolibrary.org/obo/GAZ_00014868"/>
    


    <!-- http://purl.obolibrary.org/obo/GAZ_00014869 -->

    <owl:NamedIndividual rdf:about="http://purl.obolibrary.org/obo/GAZ_00014869"/>
    


    <!-- http://purl.obolibrary.org/obo/GAZ_00014870 -->

    <owl:NamedIndividual rdf:about="http://purl.obolibrary.org/obo/GAZ_00014870"/>
    


    <!-- http://purl.obolibrary.org/obo/GAZ_00014871 -->

    <owl:NamedIndividual rdf:about="http://purl.obolibrary.org/obo/GAZ_00014871"/>
    


    <!-- http://purl.obolibrary.org/obo/GAZ_00014872 -->

    <owl:NamedIndividual rdf:about="http://purl.obolibrary.org/obo/GAZ_00014872"/>
    


    <!-- http://purl.obolibrary.org/obo/GAZ_00014873 -->

    <owl:NamedIndividual rdf:about="http://purl.obolibrary.org/obo/GAZ_00014873"/>
    


    <!-- http://purl.obolibrary.org/obo/GAZ_00014874 -->

    <owl:NamedIndividual rdf:about="http://purl.obolibrary.org/obo/GAZ_00014874"/>
    


    <!-- http://purl.obolibrary.org/obo/GAZ_00014875 -->

    <owl:NamedIndividual rdf:about="http://purl.obolibrary.org/obo/GAZ_00014875"/>
    


    <!-- http://purl.obolibrary.org/obo/GAZ_00014876 -->

    <owl:NamedIndividual rdf:about="http://purl.obolibrary.org/obo/GAZ_00014876"/>
    


    <!-- http://purl.obolibrary.org/obo/GAZ_00014877 -->

    <owl:NamedIndividual rdf:about="http://purl.obolibrary.org/obo/GAZ_00014877"/>
    


    <!-- http://purl.obolibrary.org/obo/GAZ_00014878 -->

    <owl:NamedIndividual rdf:about="http://purl.obolibrary.org/obo/GAZ_00014878"/>
    


    <!-- http://purl.obolibrary.org/obo/GAZ_00014879 -->

    <owl:NamedIndividual rdf:about="http://purl.obolibrary.org/obo/GAZ_00014879"/>
    


    <!-- http://purl.obolibrary.org/obo/GAZ_00014880 -->

    <owl:NamedIndividual rdf:about="http://purl.obolibrary.org/obo/GAZ_00014880"/>
    


    <!-- http://purl.obolibrary.org/obo/GAZ_00014881 -->

    <owl:NamedIndividual rdf:about="http://purl.obolibrary.org/obo/GAZ_00014881"/>
    


    <!-- http://purl.obolibrary.org/obo/GAZ_00014882 -->

    <owl:NamedIndividual rdf:about="http://purl.obolibrary.org/obo/GAZ_00014882"/>
    


    <!-- http://purl.obolibrary.org/obo/GAZ_00014883 -->

    <owl:NamedIndividual rdf:about="http://purl.obolibrary.org/obo/GAZ_00014883"/>
    


    <!-- http://purl.obolibrary.org/obo/GAZ_00014884 -->

    <owl:NamedIndividual rdf:about="http://purl.obolibrary.org/obo/GAZ_00014884"/>
    


    <!-- http://purl.obolibrary.org/obo/GAZ_00014885 -->

    <owl:NamedIndividual rdf:about="http://purl.obolibrary.org/obo/GAZ_00014885"/>
    


    <!-- http://purl.obolibrary.org/obo/GAZ_00014886 -->

    <owl:NamedIndividual rdf:about="http://purl.obolibrary.org/obo/GAZ_00014886"/>
    


    <!-- http://purl.obolibrary.org/obo/GAZ_00014887 -->

    <owl:NamedIndividual rdf:about="http://purl.obolibrary.org/obo/GAZ_00014887"/>
    


    <!-- http://purl.obolibrary.org/obo/GAZ_00026088 -->

    <owl:NamedIndividual rdf:about="http://purl.obolibrary.org/obo/GAZ_00026088">
        <rdf:type rdf:resource="http://purl.obolibrary.org/obo/ENVO_00000004"/>
        <obo:RO_0001025 rdf:resource="http://purl.obolibrary.org/obo/GAZ_00014880"/>
        <obo:IAO_0000115>A sum (district) of Arkhangai Province in central Mongolia.</obo:IAO_0000115>
        <oboInOwl:hasOBONamespace>GAZ</oboInOwl:hasOBONamespace>
        <oboInOwl:id>GAZ:00026088</oboInOwl:id>
        <rdfs:label>Ogii nuur District</rdfs:label>
    </owl:NamedIndividual>
    


    <!-- http://purl.obolibrary.org/obo/GAZ_00026089 -->

    <owl:NamedIndividual rdf:about="http://purl.obolibrary.org/obo/GAZ_00026089">
        <rdf:type rdf:resource="http://purl.obolibrary.org/obo/ENVO_00000004"/>
        <obo:RO_0001025 rdf:resource="http://purl.obolibrary.org/obo/GAZ_00014880"/>
        <obo:IAO_0000115>A sum (district) of Arkhangai Province in central Mongolia. Tsakhir sum lies on the extreme western edge of the aimag. On the east, it borders the sums Tariat to the north and the Khangai to the south. The western border is adjacent to Zavkhan Aimag. To the north is the Khovsgol Aimag, and to the south the Bayankhongor Aimag.</obo:IAO_0000115>
        <oboInOwl:hasOBONamespace>GAZ</oboInOwl:hasOBONamespace>
        <oboInOwl:id>GAZ:00026089</oboInOwl:id>
        <rdfs:label>Tsakhir District</rdfs:label>
    </owl:NamedIndividual>
    


    <!-- http://purl.obolibrary.org/obo/GAZ_00026090 -->

    <owl:NamedIndividual rdf:about="http://purl.obolibrary.org/obo/GAZ_00026090">
        <rdf:type rdf:resource="http://purl.obolibrary.org/obo/ENVO_00000004"/>
        <obo:RO_0001025 rdf:resource="http://purl.obolibrary.org/obo/GAZ_00014880"/>
        <obo:IAO_0000115>A sum (district) of Arkhangai Province in central Mongolia.</obo:IAO_0000115>
        <oboInOwl:hasOBONamespace>GAZ</oboInOwl:hasOBONamespace>
        <oboInOwl:id>GAZ:00026090</oboInOwl:id>
        <rdfs:label>Battsengel District</rdfs:label>
    </owl:NamedIndividual>
    


    <!-- http://purl.obolibrary.org/obo/GAZ_00026091 -->

    <owl:NamedIndividual rdf:about="http://purl.obolibrary.org/obo/GAZ_00026091">
        <rdf:type rdf:resource="http://purl.obolibrary.org/obo/ENVO_00000004"/>
        <obo:RO_0001025 rdf:resource="http://purl.obolibrary.org/obo/GAZ_00014880"/>
        <obo:IAO_0000115>A sum (district) of Arkhangai Province in central Mongolia.</obo:IAO_0000115>
        <oboInOwl:hasOBONamespace>GAZ</oboInOwl:hasOBONamespace>
        <oboInOwl:id>GAZ:00026091</oboInOwl:id>
        <rdfs:label>Tsenkher District</rdfs:label>
    </owl:NamedIndividual>
    


    <!-- http://purl.obolibrary.org/obo/GAZ_00026092 -->

    <owl:NamedIndividual rdf:about="http://purl.obolibrary.org/obo/GAZ_00026092">
        <rdf:type rdf:resource="http://purl.obolibrary.org/obo/ENVO_00000004"/>
        <obo:RO_0001025 rdf:resource="http://purl.obolibrary.org/obo/GAZ_00014880"/>
        <obo:IAO_0000115>A sum (district) of Arkhangai Province in central Mongolia.</obo:IAO_0000115>
        <oboInOwl:hasOBONamespace>GAZ</oboInOwl:hasOBONamespace>
        <oboInOwl:id>GAZ:00026092</oboInOwl:id>
        <rdfs:label>Tsetserleg District</rdfs:label>
    </owl:NamedIndividual>
    


    <!-- http://purl.obolibrary.org/obo/GAZ_00026093 -->

    <owl:NamedIndividual rdf:about="http://purl.obolibrary.org/obo/GAZ_00026093">
        <rdf:type rdf:resource="http://purl.obolibrary.org/obo/ENVO_00000004"/>
        <obo:RO_0001025 rdf:resource="http://purl.obolibrary.org/obo/GAZ_00014880"/>
        <obo:IAO_0000115>A sum (district) of Arkhangai Province in central Mongolia.</obo:IAO_0000115>
        <oboInOwl:hasOBONamespace>GAZ</oboInOwl:hasOBONamespace>
        <oboInOwl:id>GAZ:00026093</oboInOwl:id>
        <rdfs:label>Ondor-Ulaan District</rdfs:label>
    </owl:NamedIndividual>
    


    <!-- http://purl.obolibrary.org/obo/GAZ_00026094 -->

    <owl:NamedIndividual rdf:about="http://purl.obolibrary.org/obo/GAZ_00026094">
        <rdf:type rdf:resource="http://purl.obolibrary.org/obo/ENVO_00000004"/>
        <obo:RO_0001025 rdf:resource="http://purl.obolibrary.org/obo/GAZ_00014880"/>
        <obo:IAO_0000115>A sum (district) of Arkhangai Province in central Mongolia.</obo:IAO_0000115>
        <oboInOwl:hasOBONamespace>GAZ</oboInOwl:hasOBONamespace>
        <oboInOwl:id>GAZ:00026094</oboInOwl:id>
        <rdfs:label>Tariat District</rdfs:label>
    </owl:NamedIndividual>
    


    <!-- http://purl.obolibrary.org/obo/GAZ_00026095 -->

    <owl:NamedIndividual rdf:about="http://purl.obolibrary.org/obo/GAZ_00026095">
        <rdf:type rdf:resource="http://purl.obolibrary.org/obo/ENVO_00000004"/>
        <obo:RO_0001025 rdf:resource="http://purl.obolibrary.org/obo/GAZ_00014880"/>
        <obo:IAO_0000115>A sum (district) of Arkhangai Province in central Mongolia.</obo:IAO_0000115>
        <oboInOwl:hasOBONamespace>GAZ</oboInOwl:hasOBONamespace>
        <oboInOwl:id>GAZ:00026095</oboInOwl:id>
        <rdfs:label>Tuvshruulekh District</rdfs:label>
    </owl:NamedIndividual>
    


    <!-- http://purl.obolibrary.org/obo/GAZ_00026096 -->

    <owl:NamedIndividual rdf:about="http://purl.obolibrary.org/obo/GAZ_00026096">
        <rdf:type rdf:resource="http://purl.obolibrary.org/obo/ENVO_00000004"/>
        <obo:RO_0001025 rdf:resource="http://purl.obolibrary.org/obo/GAZ_00014880"/>
        <obo:IAO_0000115>A sum (district) of Arkhangai Province in central Mongolia.</obo:IAO_0000115>
        <oboInOwl:hasOBONamespace>GAZ</oboInOwl:hasOBONamespace>
        <oboInOwl:id>GAZ:00026096</oboInOwl:id>
        <rdfs:label>Ikh-Tamir District</rdfs:label>
    </owl:NamedIndividual>
    


    <!-- http://purl.obolibrary.org/obo/GAZ_00026097 -->

    <owl:NamedIndividual rdf:about="http://purl.obolibrary.org/obo/GAZ_00026097">
        <rdf:type rdf:resource="http://purl.obolibrary.org/obo/ENVO_00000004"/>
        <obo:RO_0001025 rdf:resource="http://purl.obolibrary.org/obo/GAZ_00014880"/>
        <obo:IAO_0000115>A sum (district) of Arkhangai Province in central Mongolia.</obo:IAO_0000115>
        <oboInOwl:hasOBONamespace>GAZ</oboInOwl:hasOBONamespace>
        <oboInOwl:id>GAZ:00026097</oboInOwl:id>
        <rdfs:label>Jargalant District</rdfs:label>
    </owl:NamedIndividual>
    


    <!-- http://purl.obolibrary.org/obo/GAZ_00026098 -->

    <owl:NamedIndividual rdf:about="http://purl.obolibrary.org/obo/GAZ_00026098">
        <rdf:type rdf:resource="http://purl.obolibrary.org/obo/ENVO_00000004"/>
        <obo:RO_0001025 rdf:resource="http://purl.obolibrary.org/obo/GAZ_00014880"/>
        <obo:IAO_0000115>A sum (district) of Arkhangai Province in central Mongolia.</obo:IAO_0000115>
        <oboInOwl:hasOBONamespace>GAZ</oboInOwl:hasOBONamespace>
        <oboInOwl:id>GAZ:00026098</oboInOwl:id>
        <rdfs:label>Khairkhan District</rdfs:label>
    </owl:NamedIndividual>
    


    <!-- http://purl.obolibrary.org/obo/GAZ_00026099 -->

    <owl:NamedIndividual rdf:about="http://purl.obolibrary.org/obo/GAZ_00026099">
        <rdf:type rdf:resource="http://purl.obolibrary.org/obo/ENVO_00000004"/>
        <obo:RO_0001025 rdf:resource="http://purl.obolibrary.org/obo/GAZ_00014880"/>
        <obo:IAO_0000115>A sum (district) of Arkhangai Province in central Mongolia.</obo:IAO_0000115>
        <oboInOwl:hasOBONamespace>GAZ</oboInOwl:hasOBONamespace>
        <oboInOwl:id>GAZ:00026099</oboInOwl:id>
        <rdfs:label>Khangai District</rdfs:label>
    </owl:NamedIndividual>
    


    <!-- http://purl.obolibrary.org/obo/GAZ_00026100 -->

    <owl:NamedIndividual rdf:about="http://purl.obolibrary.org/obo/GAZ_00026100">
        <rdf:type rdf:resource="http://purl.obolibrary.org/obo/ENVO_00000004"/>
        <obo:RO_0001025 rdf:resource="http://purl.obolibrary.org/obo/GAZ_00014880"/>
        <obo:IAO_0000115>A sum (district) of Arkhangai Province in central Mongolia.</obo:IAO_0000115>
        <oboInOwl:hasOBONamespace>GAZ</oboInOwl:hasOBONamespace>
        <oboInOwl:id>GAZ:00026100</oboInOwl:id>
        <rdfs:label>Erdenebulgan District</rdfs:label>
    </owl:NamedIndividual>
    


    <!-- http://purl.obolibrary.org/obo/GAZ_00026101 -->

    <owl:NamedIndividual rdf:about="http://purl.obolibrary.org/obo/GAZ_00026101">
        <rdf:type rdf:resource="http://purl.obolibrary.org/obo/ENVO_00000004"/>
        <obo:RO_0001025 rdf:resource="http://purl.obolibrary.org/obo/GAZ_00014880"/>
        <obo:IAO_0000115>A sum (district) of Arkhangai Province in central Mongolia.</obo:IAO_0000115>
        <oboInOwl:hasOBONamespace>GAZ</oboInOwl:hasOBONamespace>
        <oboInOwl:id>GAZ:00026101</oboInOwl:id>
        <rdfs:label>Chuluut District</rdfs:label>
    </owl:NamedIndividual>
    


    <!-- http://purl.obolibrary.org/obo/GAZ_00026102 -->

    <owl:NamedIndividual rdf:about="http://purl.obolibrary.org/obo/GAZ_00026102">
        <rdf:type rdf:resource="http://purl.obolibrary.org/obo/ENVO_00000004"/>
        <obo:RO_0001025 rdf:resource="http://purl.obolibrary.org/obo/GAZ_00014880"/>
        <obo:IAO_0000115>A sum (district) of Arkhangai Province in central Mongolia.</obo:IAO_0000115>
        <oboInOwl:hasOBONamespace>GAZ</oboInOwl:hasOBONamespace>
        <oboInOwl:id>GAZ:00026102</oboInOwl:id>
        <rdfs:label>Khotont District</rdfs:label>
    </owl:NamedIndividual>
    


    <!-- http://purl.obolibrary.org/obo/GAZ_00026103 -->

    <owl:NamedIndividual rdf:about="http://purl.obolibrary.org/obo/GAZ_00026103">
        <rdf:type rdf:resource="http://purl.obolibrary.org/obo/ENVO_00000004"/>
        <obo:RO_0001025 rdf:resource="http://purl.obolibrary.org/obo/GAZ_00014880"/>
        <obo:IAO_0000115>A sum (district) of Arkhangai Province in central Mongolia.</obo:IAO_0000115>
        <oboInOwl:hasOBONamespace>GAZ</oboInOwl:hasOBONamespace>
        <oboInOwl:id>GAZ:00026103</oboInOwl:id>
        <rdfs:label>Khashaat District</rdfs:label>
    </owl:NamedIndividual>
    


    <!-- http://purl.obolibrary.org/obo/GAZ_00026104 -->

    <owl:NamedIndividual rdf:about="http://purl.obolibrary.org/obo/GAZ_00026104">
        <rdf:type rdf:resource="http://purl.obolibrary.org/obo/ENVO_00000004"/>
        <obo:RO_0001025 rdf:resource="http://purl.obolibrary.org/obo/GAZ_00014880"/>
        <obo:IAO_0000115>A sum (district) of Arkhangai Province in central Mongolia.</obo:IAO_0000115>
        <oboInOwl:hasOBONamespace>GAZ</oboInOwl:hasOBONamespace>
        <oboInOwl:id>GAZ:00026104</oboInOwl:id>
        <rdfs:label>Bulgan District</rdfs:label>
    </owl:NamedIndividual>
    


    <!-- http://purl.obolibrary.org/obo/GAZ_00026105 -->

    <owl:NamedIndividual rdf:about="http://purl.obolibrary.org/obo/GAZ_00026105">
        <rdf:type rdf:resource="http://purl.obolibrary.org/obo/ENVO_00000004"/>
        <obo:RO_0001025 rdf:resource="http://purl.obolibrary.org/obo/GAZ_00014880"/>
        <obo:IAO_0000115>A sum (district) of Arkhangai Province in central Mongolia.</obo:IAO_0000115>
        <oboInOwl:hasOBONamespace>GAZ</oboInOwl:hasOBONamespace>
        <oboInOwl:id>GAZ:00026105</oboInOwl:id>
        <rdfs:label>Olziit District</rdfs:label>
    </owl:NamedIndividual>
    


    <!-- http://purl.obolibrary.org/obo/GAZ_00026106 -->

    <owl:NamedIndividual rdf:about="http://purl.obolibrary.org/obo/GAZ_00026106">
        <rdf:type rdf:resource="http://purl.obolibrary.org/obo/ENVO_00000004"/>
        <obo:RO_0001025 rdf:resource="http://purl.obolibrary.org/obo/GAZ_00014880"/>
        <obo:IAO_0000115>A sum (district) of Arkhangai Province in central Mongolia.</obo:IAO_0000115>
        <oboInOwl:hasOBONamespace>GAZ</oboInOwl:hasOBONamespace>
        <oboInOwl:id>GAZ:00026106</oboInOwl:id>
        <rdfs:label>Erdenemandal District</rdfs:label>
    </owl:NamedIndividual>
    


    <!-- http://purl.obolibrary.org/obo/GAZ_00026107 -->

    <owl:NamedIndividual rdf:about="http://purl.obolibrary.org/obo/GAZ_00026107">
        <rdf:type rdf:resource="http://purl.obolibrary.org/obo/ENVO_00000004"/>
        <obo:RO_0001025 rdf:resource="http://purl.obolibrary.org/obo/GAZ_00014878"/>
        <obo:IAO_0000115>A sum (district) of Bayan-Olgii Province in western Mongolia.</obo:IAO_0000115>
        <oboInOwl:hasOBONamespace>GAZ</oboInOwl:hasOBONamespace>
        <oboInOwl:id>GAZ:00026107</oboInOwl:id>
        <rdfs:label>Nogoonnuur District</rdfs:label>
    </owl:NamedIndividual>
    


    <!-- http://purl.obolibrary.org/obo/GAZ_00026108 -->

    <owl:NamedIndividual rdf:about="http://purl.obolibrary.org/obo/GAZ_00026108">
        <rdf:type rdf:resource="http://purl.obolibrary.org/obo/ENVO_00000004"/>
        <obo:RO_0001025 rdf:resource="http://purl.obolibrary.org/obo/GAZ_00014878"/>
        <obo:IAO_0000115>A sum (district) of Bayan-Olgii Province in western Mongolia.</obo:IAO_0000115>
        <oboInOwl:hasOBONamespace>GAZ</oboInOwl:hasOBONamespace>
        <oboInOwl:id>GAZ:00026108</oboInOwl:id>
        <rdfs:label>Tsagaannuur District</rdfs:label>
    </owl:NamedIndividual>
    


    <!-- http://purl.obolibrary.org/obo/GAZ_00026109 -->

    <owl:NamedIndividual rdf:about="http://purl.obolibrary.org/obo/GAZ_00026109">
        <rdf:type rdf:resource="http://purl.obolibrary.org/obo/ENVO_00000004"/>
        <obo:RO_0001025 rdf:resource="http://purl.obolibrary.org/obo/GAZ_00014878"/>
        <obo:IAO_0000115>A sum (district) of Bayan-Olgii Province in western Mongolia.</obo:IAO_0000115>
        <oboInOwl:hasOBONamespace>GAZ</oboInOwl:hasOBONamespace>
        <oboInOwl:id>GAZ:00026109</oboInOwl:id>
        <rdfs:label>Altai District</rdfs:label>
    </owl:NamedIndividual>
    


    <!-- http://purl.obolibrary.org/obo/GAZ_00026110 -->

    <owl:NamedIndividual rdf:about="http://purl.obolibrary.org/obo/GAZ_00026110">
        <rdf:type rdf:resource="http://purl.obolibrary.org/obo/ENVO_00000004"/>
        <obo:RO_0001025 rdf:resource="http://purl.obolibrary.org/obo/GAZ_00014878"/>
        <obo:IAO_0000115>A sum (district) of Bayan-Olgii Province in western Mongolia.</obo:IAO_0000115>
        <oboInOwl:hasOBONamespace>GAZ</oboInOwl:hasOBONamespace>
        <oboInOwl:id>GAZ:00026110</oboInOwl:id>
        <rdfs:label>Deluun District</rdfs:label>
    </owl:NamedIndividual>
    


    <!-- http://purl.obolibrary.org/obo/GAZ_00026111 -->

    <owl:NamedIndividual rdf:about="http://purl.obolibrary.org/obo/GAZ_00026111">
        <rdf:type rdf:resource="http://purl.obolibrary.org/obo/ENVO_00000004"/>
        <obo:RO_0001025 rdf:resource="http://purl.obolibrary.org/obo/GAZ_00014878"/>
        <obo:IAO_0000115>A sum (district) of Bayan-Olgii Province in western Mongolia.</obo:IAO_0000115>
        <oboInOwl:hasOBONamespace>GAZ</oboInOwl:hasOBONamespace>
        <oboInOwl:id>GAZ:00026111</oboInOwl:id>
        <rdfs:label>Tolbo District</rdfs:label>
    </owl:NamedIndividual>
    


    <!-- http://purl.obolibrary.org/obo/GAZ_00026112 -->

    <owl:NamedIndividual rdf:about="http://purl.obolibrary.org/obo/GAZ_00026112">
        <rdf:type rdf:resource="http://purl.obolibrary.org/obo/ENVO_00000004"/>
        <obo:RO_0001025 rdf:resource="http://purl.obolibrary.org/obo/GAZ_00014878"/>
        <obo:IAO_0000115>A sum (district) of Bayan-Olgii Province in western Mongolia.</obo:IAO_0000115>
        <oboInOwl:hasOBONamespace>GAZ</oboInOwl:hasOBONamespace>
        <oboInOwl:id>GAZ:00026112</oboInOwl:id>
        <rdfs:label>Bugat District</rdfs:label>
    </owl:NamedIndividual>
    


    <!-- http://purl.obolibrary.org/obo/GAZ_00026113 -->

    <owl:NamedIndividual rdf:about="http://purl.obolibrary.org/obo/GAZ_00026113">
        <rdf:type rdf:resource="http://purl.obolibrary.org/obo/ENVO_00000004"/>
        <obo:RO_0001025 rdf:resource="http://purl.obolibrary.org/obo/GAZ_00014878"/>
        <obo:IAO_0000115>A sum (district) of Bayan-Olgii Province in western Mongolia.</obo:IAO_0000115>
        <oboInOwl:hasOBONamespace>GAZ</oboInOwl:hasOBONamespace>
        <oboInOwl:id>GAZ:00026113</oboInOwl:id>
        <rdfs:label>Tsengel District</rdfs:label>
    </owl:NamedIndividual>
    


    <!-- http://purl.obolibrary.org/obo/GAZ_00026114 -->

    <owl:NamedIndividual rdf:about="http://purl.obolibrary.org/obo/GAZ_00026114">
        <rdf:type rdf:resource="http://purl.obolibrary.org/obo/ENVO_00000004"/>
        <obo:RO_0001025 rdf:resource="http://purl.obolibrary.org/obo/GAZ_00014878"/>
        <obo:IAO_0000115>A sum (district) of Bayan-Olgii Province in western Mongolia.</obo:IAO_0000115>
        <oboInOwl:hasOBONamespace>GAZ</oboInOwl:hasOBONamespace>
        <oboInOwl:id>GAZ:00026114</oboInOwl:id>
        <rdfs:label>Altantsogts District</rdfs:label>
    </owl:NamedIndividual>
    


    <!-- http://purl.obolibrary.org/obo/GAZ_00026115 -->

    <owl:NamedIndividual rdf:about="http://purl.obolibrary.org/obo/GAZ_00026115">
        <rdf:type rdf:resource="http://purl.obolibrary.org/obo/ENVO_00000004"/>
        <obo:RO_0001025 rdf:resource="http://purl.obolibrary.org/obo/GAZ_00014878"/>
        <obo:IAO_0000115>A sum (district) of Bayan-Olgii Province in western Mongolia.</obo:IAO_0000115>
        <oboInOwl:hasOBONamespace>GAZ</oboInOwl:hasOBONamespace>
        <oboInOwl:id>GAZ:00026115</oboInOwl:id>
        <rdfs:label>Sagsai District</rdfs:label>
    </owl:NamedIndividual>
    


    <!-- http://purl.obolibrary.org/obo/GAZ_00026116 -->

    <owl:NamedIndividual rdf:about="http://purl.obolibrary.org/obo/GAZ_00026116">
        <rdf:type rdf:resource="http://purl.obolibrary.org/obo/ENVO_00000004"/>
        <obo:RO_0001025 rdf:resource="http://purl.obolibrary.org/obo/GAZ_00014878"/>
        <obo:IAO_0000115>A sum (district) of Bayan-Olgii Province in western Mongolia.</obo:IAO_0000115>
        <oboInOwl:hasOBONamespace>GAZ</oboInOwl:hasOBONamespace>
        <oboInOwl:id>GAZ:00026116</oboInOwl:id>
        <rdfs:label>Buyant District</rdfs:label>
    </owl:NamedIndividual>
    


    <!-- http://purl.obolibrary.org/obo/GAZ_00026117 -->

    <owl:NamedIndividual rdf:about="http://purl.obolibrary.org/obo/GAZ_00026117">
        <obo:RO_0001025 rdf:resource="http://purl.obolibrary.org/obo/GAZ_00014878"/>
        <obo:IAO_0000115>The capital of the Bayan-Olgii Aimag (province) of Mongolia, located in the extreme west of the country.</obo:IAO_0000115>
        <oboInOwl:hasOBONamespace>GAZ</oboInOwl:hasOBONamespace>
        <oboInOwl:id>GAZ:00026117</oboInOwl:id>
        <rdfs:label>Olgii City</rdfs:label>
    </owl:NamedIndividual>
    


    <!-- http://purl.obolibrary.org/obo/GAZ_00026118 -->

    <owl:NamedIndividual rdf:about="http://purl.obolibrary.org/obo/GAZ_00026118">
        <rdf:type rdf:resource="http://purl.obolibrary.org/obo/ENVO_00000004"/>
        <obo:RO_0001025 rdf:resource="http://purl.obolibrary.org/obo/GAZ_00014878"/>
        <obo:IAO_0000115>A sum (district) of Bayan-Olgii Province in western Mongolia.</obo:IAO_0000115>
        <oboInOwl:hasOBONamespace>GAZ</oboInOwl:hasOBONamespace>
        <oboInOwl:id>GAZ:00026118</oboInOwl:id>
        <rdfs:label>Ulaankhus District</rdfs:label>
    </owl:NamedIndividual>
    


    <!-- http://purl.obolibrary.org/obo/GAZ_00026119 -->

    <owl:NamedIndividual rdf:about="http://purl.obolibrary.org/obo/GAZ_00026119">
        <rdf:type rdf:resource="http://purl.obolibrary.org/obo/ENVO_00000004"/>
        <obo:RO_0001025 rdf:resource="http://purl.obolibrary.org/obo/GAZ_00014878"/>
        <obo:IAO_0000115>A sum (district) of Bayan-Olgii Province in western Mongolia.</obo:IAO_0000115>
        <oboInOwl:hasOBONamespace>GAZ</oboInOwl:hasOBONamespace>
        <oboInOwl:id>GAZ:00026119</oboInOwl:id>
        <rdfs:label>Bayannuur District</rdfs:label>
    </owl:NamedIndividual>
    


    <!-- http://purl.obolibrary.org/obo/GAZ_00026120 -->

    <owl:NamedIndividual rdf:about="http://purl.obolibrary.org/obo/GAZ_00026120">
        <rdf:type rdf:resource="http://purl.obolibrary.org/obo/ENVO_00000004"/>
        <obo:RO_0001025 rdf:resource="http://purl.obolibrary.org/obo/GAZ_00014878"/>
        <obo:IAO_0000115>A sum (district) of Bayan-Olgii Province in western Mongolia.</obo:IAO_0000115>
        <oboInOwl:hasOBONamespace>GAZ</oboInOwl:hasOBONamespace>
        <oboInOwl:id>GAZ:00026120</oboInOwl:id>
        <rdfs:label>Bulgan District</rdfs:label>
    </owl:NamedIndividual>
    


    <!-- http://purl.obolibrary.org/obo/GAZ_00027096 -->

    <owl:NamedIndividual rdf:about="http://purl.obolibrary.org/obo/GAZ_00027096">
        <rdf:type rdf:resource="http://purl.obolibrary.org/obo/ENVO_00000004"/>
        <obo:RO_0001025 rdf:resource="http://purl.obolibrary.org/obo/GAZ_00014868"/>
        <obo:IAO_0000115>A sum (district) of Bayankhongor Province in southern Mongolia.</obo:IAO_0000115>
        <oboInOwl:hasOBONamespace>GAZ</oboInOwl:hasOBONamespace>
        <oboInOwl:id>GAZ:00027096</oboInOwl:id>
        <rdfs:label>Erdenetsogt District</rdfs:label>
    </owl:NamedIndividual>
    


    <!-- http://purl.obolibrary.org/obo/GAZ_00027097 -->

    <owl:NamedIndividual rdf:about="http://purl.obolibrary.org/obo/GAZ_00027097">
        <rdf:type rdf:resource="http://purl.obolibrary.org/obo/ENVO_00000004"/>
        <obo:RO_0001025 rdf:resource="http://purl.obolibrary.org/obo/GAZ_00014868"/>
        <obo:IAO_0000115>A sum (district) of Bayankhongor Province in southern Mongolia.</obo:IAO_0000115>
        <oboInOwl:hasOBONamespace>GAZ</oboInOwl:hasOBONamespace>
        <oboInOwl:id>GAZ:00027097</oboInOwl:id>
        <rdfs:label>Jinst District</rdfs:label>
    </owl:NamedIndividual>
    


    <!-- http://purl.obolibrary.org/obo/GAZ_00027098 -->

    <owl:NamedIndividual rdf:about="http://purl.obolibrary.org/obo/GAZ_00027098">
        <rdf:type rdf:resource="http://purl.obolibrary.org/obo/ENVO_00000004"/>
        <obo:RO_0001025 rdf:resource="http://purl.obolibrary.org/obo/GAZ_00014868"/>
        <obo:IAO_0000115>A sum (district) of Bayankhongor Province in southern Mongolia.</obo:IAO_0000115>
        <oboInOwl:hasOBONamespace>GAZ</oboInOwl:hasOBONamespace>
        <oboInOwl:id>GAZ:00027098</oboInOwl:id>
        <rdfs:label>Baatsagaan District</rdfs:label>
    </owl:NamedIndividual>
    


    <!-- http://purl.obolibrary.org/obo/GAZ_00027099 -->

    <owl:NamedIndividual rdf:about="http://purl.obolibrary.org/obo/GAZ_00027099">
        <rdf:type rdf:resource="http://purl.obolibrary.org/obo/ENVO_00000004"/>
        <obo:RO_0001025 rdf:resource="http://purl.obolibrary.org/obo/GAZ_00014868"/>
        <obo:IAO_0000115>A sum (district) of Bayankhongor Province in southern Mongolia.</obo:IAO_0000115>
        <oboInOwl:hasOBONamespace>GAZ</oboInOwl:hasOBONamespace>
        <oboInOwl:id>GAZ:00027099</oboInOwl:id>
        <rdfs:label>Buutsagaan District</rdfs:label>
    </owl:NamedIndividual>
    


    <!-- http://purl.obolibrary.org/obo/GAZ_00027100 -->

    <owl:NamedIndividual rdf:about="http://purl.obolibrary.org/obo/GAZ_00027100">
        <rdf:type rdf:resource="http://purl.obolibrary.org/obo/ENVO_00000004"/>
        <obo:RO_0001025 rdf:resource="http://purl.obolibrary.org/obo/GAZ_00014868"/>
        <obo:IAO_0000115>A sum (district) of Bayankhongor Province in southern Mongolia.</obo:IAO_0000115>
        <oboInOwl:hasOBONamespace>GAZ</oboInOwl:hasOBONamespace>
        <oboInOwl:id>GAZ:00027100</oboInOwl:id>
        <rdfs:label>Jargalant District</rdfs:label>
    </owl:NamedIndividual>
    


    <!-- http://purl.obolibrary.org/obo/GAZ_00027101 -->

    <owl:NamedIndividual rdf:about="http://purl.obolibrary.org/obo/GAZ_00027101">
        <rdf:type rdf:resource="http://purl.obolibrary.org/obo/ENVO_00000004"/>
        <obo:RO_0001025 rdf:resource="http://purl.obolibrary.org/obo/GAZ_00014868"/>
        <obo:IAO_0000115>A sum (district) of Bayankhongor Province in southern Mongolia.</obo:IAO_0000115>
        <oboInOwl:hasOBONamespace>GAZ</oboInOwl:hasOBONamespace>
        <oboInOwl:id>GAZ:00027101</oboInOwl:id>
        <rdfs:label>Bombogor District</rdfs:label>
    </owl:NamedIndividual>
    


    <!-- http://purl.obolibrary.org/obo/GAZ_00027102 -->

    <owl:NamedIndividual rdf:about="http://purl.obolibrary.org/obo/GAZ_00027102">
        <rdf:type rdf:resource="http://purl.obolibrary.org/obo/ENVO_00000004"/>
        <obo:RO_0001025 rdf:resource="http://purl.obolibrary.org/obo/GAZ_00014868"/>
        <obo:IAO_0000115>A sum (district) of Bayankhongor Province in southern Mongolia.</obo:IAO_0000115>
        <oboInOwl:hasOBONamespace>GAZ</oboInOwl:hasOBONamespace>
        <oboInOwl:id>GAZ:00027102</oboInOwl:id>
        <rdfs:label>Khureemaral District</rdfs:label>
    </owl:NamedIndividual>
    


    <!-- http://purl.obolibrary.org/obo/GAZ_00027103 -->

    <owl:NamedIndividual rdf:about="http://purl.obolibrary.org/obo/GAZ_00027103">
        <rdf:type rdf:resource="http://purl.obolibrary.org/obo/ENVO_00000004"/>
        <obo:RO_0001025 rdf:resource="http://purl.obolibrary.org/obo/GAZ_00014868"/>
        <obo:IAO_0000115>A sum (district) of Bayankhongor Province in southern Mongolia.</obo:IAO_0000115>
        <oboInOwl:hasOBONamespace>GAZ</oboInOwl:hasOBONamespace>
        <oboInOwl:id>GAZ:00027103</oboInOwl:id>
        <rdfs:label>Gurvanbulag District</rdfs:label>
    </owl:NamedIndividual>
    


    <!-- http://purl.obolibrary.org/obo/GAZ_00027104 -->

    <owl:NamedIndividual rdf:about="http://purl.obolibrary.org/obo/GAZ_00027104">
        <rdf:type rdf:resource="http://purl.obolibrary.org/obo/ENVO_00000004"/>
        <obo:RO_0001025 rdf:resource="http://purl.obolibrary.org/obo/GAZ_00014868"/>
        <obo:IAO_0000115>A sum (district) of Bayankhongor Province in southern Mongolia.</obo:IAO_0000115>
        <oboInOwl:hasOBONamespace>GAZ</oboInOwl:hasOBONamespace>
        <oboInOwl:id>GAZ:00027104</oboInOwl:id>
        <rdfs:label>Bayangovi District</rdfs:label>
    </owl:NamedIndividual>
    


    <!-- http://purl.obolibrary.org/obo/GAZ_00027105 -->

    <owl:NamedIndividual rdf:about="http://purl.obolibrary.org/obo/GAZ_00027105">
        <rdf:type rdf:resource="http://purl.obolibrary.org/obo/ENVO_00000004"/>
        <obo:RO_0001025 rdf:resource="http://purl.obolibrary.org/obo/GAZ_00014868"/>
        <obo:IAO_0000115>A sum (district) of Bayankhongor Province in southern Mongolia. The capital of the Bayankhongor Province (aimag) in Mongolia.</obo:IAO_0000115>
        <oboInOwl:hasOBONamespace>GAZ</oboInOwl:hasOBONamespace>
        <oboInOwl:id>GAZ:00027105</oboInOwl:id>
        <rdfs:label>Bayankhongor District</rdfs:label>
    </owl:NamedIndividual>
    


    <!-- http://purl.obolibrary.org/obo/GAZ_00027106 -->

    <owl:NamedIndividual rdf:about="http://purl.obolibrary.org/obo/GAZ_00027106">
        <rdf:type rdf:resource="http://purl.obolibrary.org/obo/ENVO_00000004"/>
        <obo:RO_0001025 rdf:resource="http://purl.obolibrary.org/obo/GAZ_00014868"/>
        <obo:IAO_0000115>A sum (district) of Bayankhongor Province in southern Mongolia.</obo:IAO_0000115>
        <oboInOwl:hasOBONamespace>GAZ</oboInOwl:hasOBONamespace>
        <oboInOwl:id>GAZ:00027106</oboInOwl:id>
        <rdfs:label>Bayan-Ovoo District</rdfs:label>
    </owl:NamedIndividual>
    


    <!-- http://purl.obolibrary.org/obo/GAZ_00027107 -->

    <owl:NamedIndividual rdf:about="http://purl.obolibrary.org/obo/GAZ_00027107">
        <rdf:type rdf:resource="http://purl.obolibrary.org/obo/ENVO_00000004"/>
        <obo:RO_0001025 rdf:resource="http://purl.obolibrary.org/obo/GAZ_00014868"/>
        <obo:IAO_0000115>A sum (district) of Bayankhongor Province in southern Mongolia.</obo:IAO_0000115>
        <oboInOwl:hasOBONamespace>GAZ</oboInOwl:hasOBONamespace>
        <oboInOwl:id>GAZ:00027107</oboInOwl:id>
        <rdfs:label>Bayanlig District</rdfs:label>
    </owl:NamedIndividual>
    


    <!-- http://purl.obolibrary.org/obo/GAZ_00027108 -->

    <owl:NamedIndividual rdf:about="http://purl.obolibrary.org/obo/GAZ_00027108">
        <rdf:type rdf:resource="http://purl.obolibrary.org/obo/ENVO_00000004"/>
        <obo:RO_0001025 rdf:resource="http://purl.obolibrary.org/obo/GAZ_00014868"/>
        <obo:IAO_0000115>A sum (district) of Bayankhongor Province in southern Mongolia.</obo:IAO_0000115>
        <oboInOwl:hasOBONamespace>GAZ</oboInOwl:hasOBONamespace>
        <oboInOwl:id>GAZ:00027108</oboInOwl:id>
        <rdfs:label>Bayan-Ondor District</rdfs:label>
    </owl:NamedIndividual>
    


    <!-- http://purl.obolibrary.org/obo/GAZ_00027109 -->

    <owl:NamedIndividual rdf:about="http://purl.obolibrary.org/obo/GAZ_00027109">
        <rdf:type rdf:resource="http://purl.obolibrary.org/obo/ENVO_00000004"/>
        <obo:RO_0001025 rdf:resource="http://purl.obolibrary.org/obo/GAZ_00014868"/>
        <obo:IAO_0000115>A sum (district) of Bayankhongor Province in southern Mongolia.</obo:IAO_0000115>
        <oboInOwl:hasOBONamespace>GAZ</oboInOwl:hasOBONamespace>
        <oboInOwl:id>GAZ:00027109</oboInOwl:id>
        <rdfs:label>Bayantsagaan District</rdfs:label>
    </owl:NamedIndividual>
    


    <!-- http://purl.obolibrary.org/obo/GAZ_00027110 -->

    <owl:NamedIndividual rdf:about="http://purl.obolibrary.org/obo/GAZ_00027110">
        <rdf:type rdf:resource="http://purl.obolibrary.org/obo/ENVO_00000004"/>
        <obo:RO_0001025 rdf:resource="http://purl.obolibrary.org/obo/GAZ_00014868"/>
        <obo:IAO_0000115>A sum (district) of Bayankhongor Province in southern Mongolia.</obo:IAO_0000115>
        <oboInOwl:hasOBONamespace>GAZ</oboInOwl:hasOBONamespace>
        <oboInOwl:id>GAZ:00027110</oboInOwl:id>
        <rdfs:label>Bayanbulag District</rdfs:label>
    </owl:NamedIndividual>
    


    <!-- http://purl.obolibrary.org/obo/GAZ_00027111 -->

    <owl:NamedIndividual rdf:about="http://purl.obolibrary.org/obo/GAZ_00027111">
        <rdf:type rdf:resource="http://purl.obolibrary.org/obo/ENVO_00000004"/>
        <obo:RO_0001025 rdf:resource="http://purl.obolibrary.org/obo/GAZ_00014868"/>
        <obo:IAO_0000115>A sum (district) of Bayankhongor Province in southern Mongolia.</obo:IAO_0000115>
        <oboInOwl:hasOBONamespace>GAZ</oboInOwl:hasOBONamespace>
        <oboInOwl:id>GAZ:00027111</oboInOwl:id>
        <rdfs:label>Bogd District</rdfs:label>
    </owl:NamedIndividual>
    


    <!-- http://purl.obolibrary.org/obo/GAZ_00027112 -->

    <owl:NamedIndividual rdf:about="http://purl.obolibrary.org/obo/GAZ_00027112">
        <rdf:type rdf:resource="http://purl.obolibrary.org/obo/ENVO_00000004"/>
        <obo:RO_0001025 rdf:resource="http://purl.obolibrary.org/obo/GAZ_00014868"/>
        <obo:IAO_0000115>A sum (district) of Bayankhongor Province in southern Mongolia.</obo:IAO_0000115>
        <oboInOwl:hasOBONamespace>GAZ</oboInOwl:hasOBONamespace>
        <oboInOwl:id>GAZ:00027112</oboInOwl:id>
        <rdfs:label>Galuut District</rdfs:label>
    </owl:NamedIndividual>
    


    <!-- http://purl.obolibrary.org/obo/GAZ_00027113 -->

    <owl:NamedIndividual rdf:about="http://purl.obolibrary.org/obo/GAZ_00027113">
        <rdf:type rdf:resource="http://purl.obolibrary.org/obo/ENVO_00000004"/>
        <obo:RO_0001025 rdf:resource="http://purl.obolibrary.org/obo/GAZ_00014868"/>
        <obo:IAO_0000115>A sum (district) of Bayankhongor Province in southern Mongolia.</obo:IAO_0000115>
        <oboInOwl:hasOBONamespace>GAZ</oboInOwl:hasOBONamespace>
        <oboInOwl:id>GAZ:00027113</oboInOwl:id>
        <rdfs:label>Shinejinst District</rdfs:label>
    </owl:NamedIndividual>
    


    <!-- http://purl.obolibrary.org/obo/GAZ_00027114 -->

    <owl:NamedIndividual rdf:about="http://purl.obolibrary.org/obo/GAZ_00027114">
        <rdf:type rdf:resource="http://purl.obolibrary.org/obo/ENVO_00000004"/>
        <obo:RO_0001025 rdf:resource="http://purl.obolibrary.org/obo/GAZ_00014868"/>
        <obo:IAO_0000115>A sum (district) of Bayankhongor Province in southern Mongolia.</obo:IAO_0000115>
        <oboInOwl:hasOBONamespace>GAZ</oboInOwl:hasOBONamespace>
        <oboInOwl:id>GAZ:00027114</oboInOwl:id>
        <rdfs:label>Zag District</rdfs:label>
    </owl:NamedIndividual>
    


    <!-- http://purl.obolibrary.org/obo/GAZ_00027115 -->

    <owl:NamedIndividual rdf:about="http://purl.obolibrary.org/obo/GAZ_00027115">
        <rdf:type rdf:resource="http://purl.obolibrary.org/obo/ENVO_00000004"/>
        <obo:RO_0001025 rdf:resource="http://purl.obolibrary.org/obo/GAZ_00014868"/>
        <obo:IAO_0000115>A sum (district) of Bayankhongor Province in southern Mongolia.</obo:IAO_0000115>
        <oboInOwl:hasOBONamespace>GAZ</oboInOwl:hasOBONamespace>
        <oboInOwl:id>GAZ:00027115</oboInOwl:id>
        <rdfs:label>Olziit District</rdfs:label>
    </owl:NamedIndividual>
    


    <!-- http://purl.obolibrary.org/obo/GAZ_00027116 -->

    <owl:NamedIndividual rdf:about="http://purl.obolibrary.org/obo/GAZ_00027116">
        <rdf:type rdf:resource="http://purl.obolibrary.org/obo/ENVO_00000004"/>
        <obo:RO_0001025 rdf:resource="http://purl.obolibrary.org/obo/GAZ_00014874"/>
        <obo:IAO_0000115>A sum (district) of Bulgan Province in northern Mongolia.</obo:IAO_0000115>
        <oboInOwl:hasOBONamespace>GAZ</oboInOwl:hasOBONamespace>
        <oboInOwl:id>GAZ:00027116</oboInOwl:id>
        <rdfs:label>Dashinchilen District</rdfs:label>
    </owl:NamedIndividual>
    


    <!-- http://purl.obolibrary.org/obo/GAZ_00027117 -->

    <owl:NamedIndividual rdf:about="http://purl.obolibrary.org/obo/GAZ_00027117">
        <rdf:type rdf:resource="http://purl.obolibrary.org/obo/ENVO_00000004"/>
        <obo:RO_0001025 rdf:resource="http://purl.obolibrary.org/obo/GAZ_00014874"/>
        <obo:IAO_0000115>A sum (district) of Bulgan Province in northern Mongolia.</obo:IAO_0000115>
        <oboInOwl:hasOBONamespace>GAZ</oboInOwl:hasOBONamespace>
        <oboInOwl:id>GAZ:00027117</oboInOwl:id>
        <rdfs:label>Bugat District</rdfs:label>
    </owl:NamedIndividual>
    


    <!-- http://purl.obolibrary.org/obo/GAZ_00027118 -->

    <owl:NamedIndividual rdf:about="http://purl.obolibrary.org/obo/GAZ_00027118">
        <rdf:type rdf:resource="http://purl.obolibrary.org/obo/ENVO_00000004"/>
        <obo:RO_0001025 rdf:resource="http://purl.obolibrary.org/obo/GAZ_00014874"/>
        <obo:IAO_0000115>A sum (district) of Bulgan Province in northern Mongolia.</obo:IAO_0000115>
        <oboInOwl:hasOBONamespace>GAZ</oboInOwl:hasOBONamespace>
        <oboInOwl:id>GAZ:00027118</oboInOwl:id>
        <rdfs:label>Buregkhangai District</rdfs:label>
    </owl:NamedIndividual>
    


    <!-- http://purl.obolibrary.org/obo/GAZ_00027119 -->

    <owl:NamedIndividual rdf:about="http://purl.obolibrary.org/obo/GAZ_00027119">
        <rdf:type rdf:resource="http://purl.obolibrary.org/obo/ENVO_00000004"/>
        <obo:RO_0001025 rdf:resource="http://purl.obolibrary.org/obo/GAZ_00014874"/>
        <obo:IAO_0000115>A sum (district) of Bulgan Province in northern Mongolia.</obo:IAO_0000115>
        <oboInOwl:hasOBONamespace>GAZ</oboInOwl:hasOBONamespace>
        <oboInOwl:id>GAZ:00027119</oboInOwl:id>
        <rdfs:label>Bayannuur District</rdfs:label>
    </owl:NamedIndividual>
    


    <!-- http://purl.obolibrary.org/obo/GAZ_00027120 -->

    <owl:NamedIndividual rdf:about="http://purl.obolibrary.org/obo/GAZ_00027120">
        <rdf:type rdf:resource="http://purl.obolibrary.org/obo/ENVO_00000004"/>
        <obo:RO_0001025 rdf:resource="http://purl.obolibrary.org/obo/GAZ_00014874"/>
        <obo:IAO_0000115>A sum (district) of Bulgan Province in northern Mongolia.</obo:IAO_0000115>
        <oboInOwl:hasOBONamespace>GAZ</oboInOwl:hasOBONamespace>
        <oboInOwl:id>GAZ:00027120</oboInOwl:id>
        <rdfs:label>Bayan-Agt District</rdfs:label>
    </owl:NamedIndividual>
    


    <!-- http://purl.obolibrary.org/obo/GAZ_00027121 -->

    <owl:NamedIndividual rdf:about="http://purl.obolibrary.org/obo/GAZ_00027121">
        <rdf:type rdf:resource="http://purl.obolibrary.org/obo/ENVO_00000004"/>
        <obo:RO_0001025 rdf:resource="http://purl.obolibrary.org/obo/GAZ_00014874"/>
        <obo:IAO_0000115>A sum (district) of Bulgan Province in northern Mongolia.</obo:IAO_0000115>
        <oboInOwl:hasOBONamespace>GAZ</oboInOwl:hasOBONamespace>
        <oboInOwl:id>GAZ:00027121</oboInOwl:id>
        <rdfs:label>Khangal District</rdfs:label>
    </owl:NamedIndividual>
    


    <!-- http://purl.obolibrary.org/obo/GAZ_00027122 -->

    <owl:NamedIndividual rdf:about="http://purl.obolibrary.org/obo/GAZ_00027122">
        <rdf:type rdf:resource="http://purl.obolibrary.org/obo/ENVO_00000004"/>
        <obo:RO_0001025 rdf:resource="http://purl.obolibrary.org/obo/GAZ_00014874"/>
        <obo:IAO_0000115>A sum (district) of Bulgan Province in northern Mongolia.</obo:IAO_0000115>
        <oboInOwl:hasOBONamespace>GAZ</oboInOwl:hasOBONamespace>
        <oboInOwl:id>GAZ:00027122</oboInOwl:id>
        <rdfs:label>Saikhan District</rdfs:label>
    </owl:NamedIndividual>
    


    <!-- http://purl.obolibrary.org/obo/GAZ_00027123 -->

    <owl:NamedIndividual rdf:about="http://purl.obolibrary.org/obo/GAZ_00027123">
        <rdf:type rdf:resource="http://purl.obolibrary.org/obo/ENVO_00000004"/>
        <obo:RO_0001025 rdf:resource="http://purl.obolibrary.org/obo/GAZ_00014874"/>
        <obo:IAO_0000115>A sum (district) of Bulgan Province in northern Mongolia.</obo:IAO_0000115>
        <oboInOwl:hasOBONamespace>GAZ</oboInOwl:hasOBONamespace>
        <oboInOwl:id>GAZ:00027123</oboInOwl:id>
        <rdfs:label>Gurvanbulag District</rdfs:label>
    </owl:NamedIndividual>
    


    <!-- http://purl.obolibrary.org/obo/GAZ_00027124 -->

    <owl:NamedIndividual rdf:about="http://purl.obolibrary.org/obo/GAZ_00027124">
        <rdf:type rdf:resource="http://purl.obolibrary.org/obo/ENVO_00000004"/>
        <obo:RO_0001025 rdf:resource="http://purl.obolibrary.org/obo/GAZ_00014874"/>
        <obo:IAO_0000115>A sum (district) of Bulgan Province in northern Mongolia.</obo:IAO_0000115>
        <oboInOwl:hasOBONamespace>GAZ</oboInOwl:hasOBONamespace>
        <oboInOwl:id>GAZ:00027124</oboInOwl:id>
        <rdfs:label>Khutag-Ondor District</rdfs:label>
    </owl:NamedIndividual>
    


    <!-- http://purl.obolibrary.org/obo/GAZ_00027125 -->

    <owl:NamedIndividual rdf:about="http://purl.obolibrary.org/obo/GAZ_00027125">
        <rdf:type rdf:resource="http://purl.obolibrary.org/obo/ENVO_00000004"/>
        <obo:RO_0001025 rdf:resource="http://purl.obolibrary.org/obo/GAZ_00014874"/>
        <obo:IAO_0000115>A sum (district) of Bulgan Province in northern Mongolia.</obo:IAO_0000115>
        <oboInOwl:hasOBONamespace>GAZ</oboInOwl:hasOBONamespace>
        <oboInOwl:id>GAZ:00027125</oboInOwl:id>
        <rdfs:label>Rashaant District</rdfs:label>
    </owl:NamedIndividual>
    


    <!-- http://purl.obolibrary.org/obo/GAZ_00027126 -->

    <owl:NamedIndividual rdf:about="http://purl.obolibrary.org/obo/GAZ_00027126">
        <rdf:type rdf:resource="http://purl.obolibrary.org/obo/ENVO_00000004"/>
        <obo:RO_0001025 rdf:resource="http://purl.obolibrary.org/obo/GAZ_00014874"/>
        <obo:IAO_0000115>A sum (district) of Bulgan Province in northern Mongolia.</obo:IAO_0000115>
        <oboInOwl:hasOBONamespace>GAZ</oboInOwl:hasOBONamespace>
        <oboInOwl:id>GAZ:00027126</oboInOwl:id>
        <rdfs:label>Orkhon District</rdfs:label>
    </owl:NamedIndividual>
    


    <!-- http://purl.obolibrary.org/obo/GAZ_00027127 -->

    <owl:NamedIndividual rdf:about="http://purl.obolibrary.org/obo/GAZ_00027127">
        <rdf:type rdf:resource="http://purl.obolibrary.org/obo/ENVO_00000004"/>
        <obo:RO_0001025 rdf:resource="http://purl.obolibrary.org/obo/GAZ_00014874"/>
        <obo:IAO_0000115>A sum (district) of Bulgan Province in northern Mongolia.</obo:IAO_0000115>
        <oboInOwl:hasOBONamespace>GAZ</oboInOwl:hasOBONamespace>
        <oboInOwl:id>GAZ:00027127</oboInOwl:id>
        <rdfs:label>Teshig District</rdfs:label>
    </owl:NamedIndividual>
    


    <!-- http://purl.obolibrary.org/obo/GAZ_00027128 -->

    <owl:NamedIndividual rdf:about="http://purl.obolibrary.org/obo/GAZ_00027128">
        <rdf:type rdf:resource="http://purl.obolibrary.org/obo/ENVO_00000004"/>
        <obo:RO_0001025 rdf:resource="http://purl.obolibrary.org/obo/GAZ_00014874"/>
        <obo:IAO_0000115>A sum (district) of Bulgan Province in northern Mongolia.</obo:IAO_0000115>
        <oboInOwl:hasOBONamespace>GAZ</oboInOwl:hasOBONamespace>
        <oboInOwl:id>GAZ:00027128</oboInOwl:id>
        <rdfs:label>Khishig-Ondor District</rdfs:label>
    </owl:NamedIndividual>
    


    <!-- http://purl.obolibrary.org/obo/GAZ_00027129 -->

    <owl:NamedIndividual rdf:about="http://purl.obolibrary.org/obo/GAZ_00027129">
        <rdf:type rdf:resource="http://purl.obolibrary.org/obo/ENVO_00000004"/>
        <obo:RO_0001025 rdf:resource="http://purl.obolibrary.org/obo/GAZ_00014874"/>
        <obo:IAO_0000115>A sum (district) of Bulgan Province in northern Mongolia. The capital city of Mongolia&apos;s Bulgan province.</obo:IAO_0000115>
        <oboInOwl:hasOBONamespace>GAZ</oboInOwl:hasOBONamespace>
        <oboInOwl:id>GAZ:00027129</oboInOwl:id>
        <rdfs:label>Bulgan City</rdfs:label>
    </owl:NamedIndividual>
    


    <!-- http://purl.obolibrary.org/obo/GAZ_00027130 -->

    <owl:NamedIndividual rdf:about="http://purl.obolibrary.org/obo/GAZ_00027130">
        <rdf:type rdf:resource="http://purl.obolibrary.org/obo/ENVO_00000004"/>
        <obo:RO_0001025 rdf:resource="http://purl.obolibrary.org/obo/GAZ_00014874"/>
        <obo:IAO_0000115>A sum (district) of Bulgan Province in northern Mongolia.</obo:IAO_0000115>
        <oboInOwl:hasOBONamespace>GAZ</oboInOwl:hasOBONamespace>
        <oboInOwl:id>GAZ:00027130</oboInOwl:id>
        <rdfs:label>Mogod District</rdfs:label>
    </owl:NamedIndividual>
    


    <!-- http://purl.obolibrary.org/obo/GAZ_00027131 -->

    <owl:NamedIndividual rdf:about="http://purl.obolibrary.org/obo/GAZ_00027131">
        <rdf:type rdf:resource="http://purl.obolibrary.org/obo/ENVO_00000004"/>
        <obo:RO_0001025 rdf:resource="http://purl.obolibrary.org/obo/GAZ_00014874"/>
        <obo:IAO_0000115>A sum (district) of Bulgan Province in northern Mongolia.</obo:IAO_0000115>
        <oboInOwl:hasOBONamespace>GAZ</oboInOwl:hasOBONamespace>
        <oboInOwl:id>GAZ:00027131</oboInOwl:id>
        <rdfs:label>Selenge District</rdfs:label>
    </owl:NamedIndividual>
    


    <!-- http://purl.obolibrary.org/obo/GAZ_00027132 -->

    <owl:NamedIndividual rdf:about="http://purl.obolibrary.org/obo/GAZ_00027132">
        <rdf:type rdf:resource="http://purl.obolibrary.org/obo/ENVO_00000004"/>
        <obo:RO_0001025 rdf:resource="http://purl.obolibrary.org/obo/GAZ_00014872"/>
        <obo:IAO_0000115>A sum (district) of Darkhan-Uul Province in northern Mongolia.</obo:IAO_0000115>
        <oboInOwl:hasOBONamespace>GAZ</oboInOwl:hasOBONamespace>
        <oboInOwl:id>GAZ:00027132</oboInOwl:id>
        <rdfs:label>Khongor District</rdfs:label>
    </owl:NamedIndividual>
    


    <!-- http://purl.obolibrary.org/obo/GAZ_00027133 -->

    <owl:NamedIndividual rdf:about="http://purl.obolibrary.org/obo/GAZ_00027133">
        <obo:RO_0001025 rdf:resource="http://purl.obolibrary.org/obo/GAZ_00014872"/>
        <obo:IAO_0000115>The third-largest city in Mongolia and the capital of Darkhan-Uul Aimag (Darkhan-Uul Province).</obo:IAO_0000115>
        <oboInOwl:hasOBONamespace>GAZ</oboInOwl:hasOBONamespace>
        <oboInOwl:id>GAZ:00027133</oboInOwl:id>
        <rdfs:label>Darkhan City</rdfs:label>
    </owl:NamedIndividual>
    


    <!-- http://purl.obolibrary.org/obo/GAZ_00027134 -->

    <owl:NamedIndividual rdf:about="http://purl.obolibrary.org/obo/GAZ_00027134">
        <rdf:type rdf:resource="http://purl.obolibrary.org/obo/ENVO_00000004"/>
        <obo:RO_0001025 rdf:resource="http://purl.obolibrary.org/obo/GAZ_00014872"/>
        <obo:IAO_0000115>A sum (district) of Darkhan-Uul Province in northern Mongolia.</obo:IAO_0000115>
        <oboInOwl:hasOBONamespace>GAZ</oboInOwl:hasOBONamespace>
        <oboInOwl:id>GAZ:00027134</oboInOwl:id>
        <rdfs:label>Sharyngol District</rdfs:label>
    </owl:NamedIndividual>
    


    <!-- http://purl.obolibrary.org/obo/GAZ_00027135 -->

    <owl:NamedIndividual rdf:about="http://purl.obolibrary.org/obo/GAZ_00027135">
        <rdf:type rdf:resource="http://purl.obolibrary.org/obo/ENVO_00000004"/>
        <obo:RO_0001025 rdf:resource="http://purl.obolibrary.org/obo/GAZ_00014872"/>
        <obo:IAO_0000115>A sum (district) of Darkhan-Uul Province in northern Mongolia.</obo:IAO_0000115>
        <oboInOwl:hasOBONamespace>GAZ</oboInOwl:hasOBONamespace>
        <oboInOwl:id>GAZ:00027135</oboInOwl:id>
        <rdfs:label>Orkhon District</rdfs:label>
    </owl:NamedIndividual>
    


    <!-- http://purl.obolibrary.org/obo/GAZ_00027136 -->

    <owl:NamedIndividual rdf:about="http://purl.obolibrary.org/obo/GAZ_00027136">
        <rdf:type rdf:resource="http://purl.obolibrary.org/obo/ENVO_00000004"/>
        <obo:RO_0001025 rdf:resource="http://purl.obolibrary.org/obo/GAZ_00014875"/>
        <obo:IAO_0000115>A sum (district) of Dornod Province in eastern Mongolia.</obo:IAO_0000115>
        <oboInOwl:hasOBONamespace>GAZ</oboInOwl:hasOBONamespace>
        <oboInOwl:id>GAZ:00027136</oboInOwl:id>
        <rdfs:label>Khalkhgol District</rdfs:label>
    </owl:NamedIndividual>
    


    <!-- http://purl.obolibrary.org/obo/GAZ_00027137 -->

    <owl:NamedIndividual rdf:about="http://purl.obolibrary.org/obo/GAZ_00027137">
        <rdf:type rdf:resource="http://purl.obolibrary.org/obo/ENVO_00000004"/>
        <obo:RO_0001025 rdf:resource="http://purl.obolibrary.org/obo/GAZ_00014875"/>
        <obo:IAO_0000115>A sum (district) of Dornod Province in eastern Mongolia.</obo:IAO_0000115>
        <oboInOwl:hasOBONamespace>GAZ</oboInOwl:hasOBONamespace>
        <oboInOwl:id>GAZ:00027137</oboInOwl:id>
        <rdfs:label>Matad District</rdfs:label>
    </owl:NamedIndividual>
    


    <!-- http://purl.obolibrary.org/obo/GAZ_00027138 -->

    <owl:NamedIndividual rdf:about="http://purl.obolibrary.org/obo/GAZ_00027138">
        <rdf:type rdf:resource="http://purl.obolibrary.org/obo/ENVO_00000004"/>
        <obo:RO_0001025 rdf:resource="http://purl.obolibrary.org/obo/GAZ_00014875"/>
        <obo:IAO_0000115>A sum (district) of Dornod Province in eastern Mongolia.</obo:IAO_0000115>
        <oboInOwl:hasOBONamespace>GAZ</oboInOwl:hasOBONamespace>
        <oboInOwl:id>GAZ:00027138</oboInOwl:id>
        <rdfs:label>Bayandun District</rdfs:label>
    </owl:NamedIndividual>
    


    <!-- http://purl.obolibrary.org/obo/GAZ_00027139 -->

    <owl:NamedIndividual rdf:about="http://purl.obolibrary.org/obo/GAZ_00027139">
        <rdf:type rdf:resource="http://purl.obolibrary.org/obo/ENVO_00000004"/>
        <obo:RO_0001025 rdf:resource="http://purl.obolibrary.org/obo/GAZ_00014875"/>
        <obo:IAO_0000115>A sum (district) of Dornod Province in eastern Mongolia.</obo:IAO_0000115>
        <oboInOwl:hasOBONamespace>GAZ</oboInOwl:hasOBONamespace>
        <oboInOwl:id>GAZ:00027139</oboInOwl:id>
        <rdfs:label>Gurvanzagal District</rdfs:label>
    </owl:NamedIndividual>
    


    <!-- http://purl.obolibrary.org/obo/GAZ_00027140 -->

    <owl:NamedIndividual rdf:about="http://purl.obolibrary.org/obo/GAZ_00027140">
        <rdf:type rdf:resource="http://purl.obolibrary.org/obo/ENVO_00000004"/>
        <obo:RO_0001025 rdf:resource="http://purl.obolibrary.org/obo/GAZ_00014875"/>
        <obo:IAO_0000115>A sum (district) of Dornod Province in eastern Mongolia.</obo:IAO_0000115>
        <oboInOwl:hasOBONamespace>GAZ</oboInOwl:hasOBONamespace>
        <oboInOwl:id>GAZ:00027140</oboInOwl:id>
        <rdfs:label>Sergelen District</rdfs:label>
    </owl:NamedIndividual>
    


    <!-- http://purl.obolibrary.org/obo/GAZ_00027141 -->

    <owl:NamedIndividual rdf:about="http://purl.obolibrary.org/obo/GAZ_00027141">
        <rdf:type rdf:resource="http://purl.obolibrary.org/obo/ENVO_00000004"/>
        <obo:RO_0001025 rdf:resource="http://purl.obolibrary.org/obo/GAZ_00014875"/>
        <obo:IAO_0000115>A sum (district) of Dornod Province in eastern Mongolia.</obo:IAO_0000115>
        <oboInOwl:hasOBONamespace>GAZ</oboInOwl:hasOBONamespace>
        <oboInOwl:id>GAZ:00027141</oboInOwl:id>
        <rdfs:label>Kherlen District</rdfs:label>
    </owl:NamedIndividual>
    


    <!-- http://purl.obolibrary.org/obo/GAZ_00027142 -->

    <owl:NamedIndividual rdf:about="http://purl.obolibrary.org/obo/GAZ_00027142">
        <rdf:type rdf:resource="http://purl.obolibrary.org/obo/ENVO_00000004"/>
        <obo:RO_0001025 rdf:resource="http://purl.obolibrary.org/obo/GAZ_00014875"/>
        <obo:IAO_0000115>A sum (district) of Dornod Province in eastern Mongolia.</obo:IAO_0000115>
        <oboInOwl:hasOBONamespace>GAZ</oboInOwl:hasOBONamespace>
        <oboInOwl:id>GAZ:00027142</oboInOwl:id>
        <rdfs:label>Bayantumen District</rdfs:label>
    </owl:NamedIndividual>
    


    <!-- http://purl.obolibrary.org/obo/GAZ_00027143 -->

    <owl:NamedIndividual rdf:about="http://purl.obolibrary.org/obo/GAZ_00027143">
        <rdf:type rdf:resource="http://purl.obolibrary.org/obo/ENVO_00000004"/>
        <obo:RO_0001025 rdf:resource="http://purl.obolibrary.org/obo/GAZ_00014875"/>
        <obo:IAO_0000115>A sum (district) of Dornod Province in eastern Mongolia.</obo:IAO_0000115>
        <oboInOwl:hasOBONamespace>GAZ</oboInOwl:hasOBONamespace>
        <oboInOwl:id>GAZ:00027143</oboInOwl:id>
        <rdfs:label>Chuluunkhoroot District</rdfs:label>
    </owl:NamedIndividual>
    


    <!-- http://purl.obolibrary.org/obo/GAZ_00027144 -->

    <owl:NamedIndividual rdf:about="http://purl.obolibrary.org/obo/GAZ_00027144">
        <rdf:type rdf:resource="http://purl.obolibrary.org/obo/ENVO_00000004"/>
        <obo:RO_0001025 rdf:resource="http://purl.obolibrary.org/obo/GAZ_00014875"/>
        <obo:IAO_0000115>A sum (district) of Dornod Province in eastern Mongolia.</obo:IAO_0000115>
        <oboInOwl:hasOBONamespace>GAZ</oboInOwl:hasOBONamespace>
        <oboInOwl:id>GAZ:00027144</oboInOwl:id>
        <rdfs:label>Choibalsan District</rdfs:label>
    </owl:NamedIndividual>
    


    <!-- http://purl.obolibrary.org/obo/GAZ_00027145 -->

    <owl:NamedIndividual rdf:about="http://purl.obolibrary.org/obo/GAZ_00027145">
        <rdf:type rdf:resource="http://purl.obolibrary.org/obo/ENVO_00000004"/>
        <obo:RO_0001025 rdf:resource="http://purl.obolibrary.org/obo/GAZ_00014875"/>
        <obo:IAO_0000115>A sum (district) of Dornod Province in eastern Mongolia.</obo:IAO_0000115>
        <oboInOwl:hasOBONamespace>GAZ</oboInOwl:hasOBONamespace>
        <oboInOwl:id>GAZ:00027145</oboInOwl:id>
        <rdfs:label>Kholonbuir District</rdfs:label>
    </owl:NamedIndividual>
    


    <!-- http://purl.obolibrary.org/obo/GAZ_00027146 -->

    <owl:NamedIndividual rdf:about="http://purl.obolibrary.org/obo/GAZ_00027146">
        <rdf:type rdf:resource="http://purl.obolibrary.org/obo/ENVO_00000004"/>
        <obo:RO_0001025 rdf:resource="http://purl.obolibrary.org/obo/GAZ_00014875"/>
        <obo:IAO_0000115>A sum (district) of Dornod Province in eastern Mongolia.</obo:IAO_0000115>
        <oboInOwl:hasOBONamespace>GAZ</oboInOwl:hasOBONamespace>
        <oboInOwl:id>GAZ:00027146</oboInOwl:id>
        <rdfs:label>Bayan-Uul District</rdfs:label>
    </owl:NamedIndividual>
    


    <!-- http://purl.obolibrary.org/obo/GAZ_00027147 -->

    <owl:NamedIndividual rdf:about="http://purl.obolibrary.org/obo/GAZ_00027147">
        <rdf:type rdf:resource="http://purl.obolibrary.org/obo/ENVO_00000004"/>
        <obo:RO_0001025 rdf:resource="http://purl.obolibrary.org/obo/GAZ_00014875"/>
        <obo:IAO_0000115>A sum (district) of Dornod Province in eastern Mongolia.</obo:IAO_0000115>
        <oboInOwl:hasOBONamespace>GAZ</oboInOwl:hasOBONamespace>
        <oboInOwl:id>GAZ:00027147</oboInOwl:id>
        <rdfs:label>Bulgan District</rdfs:label>
    </owl:NamedIndividual>
    


    <!-- http://purl.obolibrary.org/obo/GAZ_00027148 -->

    <owl:NamedIndividual rdf:about="http://purl.obolibrary.org/obo/GAZ_00027148">
        <rdf:type rdf:resource="http://purl.obolibrary.org/obo/ENVO_00000004"/>
        <obo:RO_0001025 rdf:resource="http://purl.obolibrary.org/obo/GAZ_00014875"/>
        <obo:IAO_0000115>A sum (district) of Dornod Province in eastern Mongolia.</obo:IAO_0000115>
        <oboInOwl:hasOBONamespace>GAZ</oboInOwl:hasOBONamespace>
        <oboInOwl:id>GAZ:00027148</oboInOwl:id>
        <rdfs:label>Dashbalbar District</rdfs:label>
    </owl:NamedIndividual>
    


    <!-- http://purl.obolibrary.org/obo/GAZ_00027149 -->

    <owl:NamedIndividual rdf:about="http://purl.obolibrary.org/obo/GAZ_00027149">
        <rdf:type rdf:resource="http://purl.obolibrary.org/obo/ENVO_00000004"/>
        <obo:RO_0001025 rdf:resource="http://purl.obolibrary.org/obo/GAZ_00014875"/>
        <obo:IAO_0000115>A sum (district) of Dornod Province in eastern Mongolia.</obo:IAO_0000115>
        <oboInOwl:hasOBONamespace>GAZ</oboInOwl:hasOBONamespace>
        <oboInOwl:id>GAZ:00027149</oboInOwl:id>
        <rdfs:label>Tsagaan-Ovoo District</rdfs:label>
    </owl:NamedIndividual>
    


    <!-- http://purl.obolibrary.org/obo/GAZ_00027150 -->

    <owl:NamedIndividual rdf:about="http://purl.obolibrary.org/obo/GAZ_00027150">
        <rdf:type rdf:resource="http://purl.obolibrary.org/obo/ENVO_00000004"/>
        <obo:RO_0001025 rdf:resource="http://purl.obolibrary.org/obo/GAZ_00014870"/>
        <obo:IAO_0000115>A sum (district) of Dornogovi Province in southeastern Mongolia.</obo:IAO_0000115>
        <oboInOwl:hasOBONamespace>GAZ</oboInOwl:hasOBONamespace>
        <oboInOwl:id>GAZ:00027150</oboInOwl:id>
        <rdfs:label>Khovsgol District</rdfs:label>
    </owl:NamedIndividual>
    


    <!-- http://purl.obolibrary.org/obo/GAZ_00027151 -->

    <owl:NamedIndividual rdf:about="http://purl.obolibrary.org/obo/GAZ_00027151">
        <rdf:type rdf:resource="http://purl.obolibrary.org/obo/ENVO_00000004"/>
        <obo:RO_0001025 rdf:resource="http://purl.obolibrary.org/obo/GAZ_00014870"/>
        <obo:IAO_0000115>A sum (district) of Dornogovi Province in southeastern Mongolia.</obo:IAO_0000115>
        <oboInOwl:hasOBONamespace>GAZ</oboInOwl:hasOBONamespace>
        <oboInOwl:id>GAZ:00027151</oboInOwl:id>
        <rdfs:label>Zamyn-Uud District</rdfs:label>
    </owl:NamedIndividual>
    


    <!-- http://purl.obolibrary.org/obo/GAZ_00027152 -->

    <owl:NamedIndividual rdf:about="http://purl.obolibrary.org/obo/GAZ_00027152">
        <rdf:type rdf:resource="http://purl.obolibrary.org/obo/ENVO_00000004"/>
        <obo:RO_0001025 rdf:resource="http://purl.obolibrary.org/obo/GAZ_00014870"/>
        <obo:IAO_0000115>A sum (district) of Dornogovi Province in southeastern Mongolia.</obo:IAO_0000115>
        <oboInOwl:hasOBONamespace>GAZ</oboInOwl:hasOBONamespace>
        <oboInOwl:id>GAZ:00027152</oboInOwl:id>
        <rdfs:label>Altanshiree District</rdfs:label>
    </owl:NamedIndividual>
    


    <!-- http://purl.obolibrary.org/obo/GAZ_00027153 -->

    <owl:NamedIndividual rdf:about="http://purl.obolibrary.org/obo/GAZ_00027153">
        <rdf:type rdf:resource="http://purl.obolibrary.org/obo/ENVO_00000004"/>
        <obo:RO_0001025 rdf:resource="http://purl.obolibrary.org/obo/GAZ_00014870"/>
        <obo:IAO_0000115>A sum (district) of Dornogovi Province in southeastern Mongolia.</obo:IAO_0000115>
        <oboInOwl:hasOBONamespace>GAZ</oboInOwl:hasOBONamespace>
        <oboInOwl:id>GAZ:00027153</oboInOwl:id>
        <rdfs:label>Ulaanbadrakh District</rdfs:label>
    </owl:NamedIndividual>
    


    <!-- http://purl.obolibrary.org/obo/GAZ_00027154 -->

    <owl:NamedIndividual rdf:about="http://purl.obolibrary.org/obo/GAZ_00027154">
        <rdf:type rdf:resource="http://purl.obolibrary.org/obo/ENVO_00000004"/>
        <obo:RO_0001025 rdf:resource="http://purl.obolibrary.org/obo/GAZ_00014870"/>
        <obo:IAO_0000115>A sum (district) of Dornogovi Province in southeastern Mongolia.</obo:IAO_0000115>
        <oboInOwl:hasOBONamespace>GAZ</oboInOwl:hasOBONamespace>
        <oboInOwl:id>GAZ:00027154</oboInOwl:id>
        <rdfs:label>Orgon District</rdfs:label>
    </owl:NamedIndividual>
    


    <!-- http://purl.obolibrary.org/obo/GAZ_00027155 -->

    <owl:NamedIndividual rdf:about="http://purl.obolibrary.org/obo/GAZ_00027155">
        <rdf:type rdf:resource="http://purl.obolibrary.org/obo/ENVO_00000004"/>
        <obo:RO_0001025 rdf:resource="http://purl.obolibrary.org/obo/GAZ_00014870"/>
        <obo:IAO_0000115>A sum (district) of Dornogovi Province in southeastern Mongolia.</obo:IAO_0000115>
        <oboInOwl:hasOBONamespace>GAZ</oboInOwl:hasOBONamespace>
        <oboInOwl:id>GAZ:00027155</oboInOwl:id>
        <rdfs:label>Erdene District</rdfs:label>
    </owl:NamedIndividual>
    


    <!-- http://purl.obolibrary.org/obo/GAZ_00027156 -->

    <owl:NamedIndividual rdf:about="http://purl.obolibrary.org/obo/GAZ_00027156">
        <rdf:type rdf:resource="http://purl.obolibrary.org/obo/ENVO_00000004"/>
        <obo:RO_0001025 rdf:resource="http://purl.obolibrary.org/obo/GAZ_00014870"/>
        <obo:IAO_0000115>A sum (district) of Dornogovi Province in southeastern Mongolia.</obo:IAO_0000115>
        <oboInOwl:hasOBONamespace>GAZ</oboInOwl:hasOBONamespace>
        <oboInOwl:id>GAZ:00027156</oboInOwl:id>
        <rdfs:label>Sainshand District</rdfs:label>
    </owl:NamedIndividual>
    


    <!-- http://purl.obolibrary.org/obo/GAZ_00027157 -->

    <owl:NamedIndividual rdf:about="http://purl.obolibrary.org/obo/GAZ_00027157">
        <rdf:type rdf:resource="http://purl.obolibrary.org/obo/ENVO_00000004"/>
        <obo:RO_0001025 rdf:resource="http://purl.obolibrary.org/obo/GAZ_00014870"/>
        <obo:IAO_0000115>A sum (district) of Dornogovi Province in southeastern Mongolia.</obo:IAO_0000115>
        <oboInOwl:hasOBONamespace>GAZ</oboInOwl:hasOBONamespace>
        <oboInOwl:id>GAZ:00027157</oboInOwl:id>
        <rdfs:label>Saikhandulaan District</rdfs:label>
    </owl:NamedIndividual>
    


    <!-- http://purl.obolibrary.org/obo/GAZ_00027158 -->

    <owl:NamedIndividual rdf:about="http://purl.obolibrary.org/obo/GAZ_00027158">
        <rdf:type rdf:resource="http://purl.obolibrary.org/obo/ENVO_00000004"/>
        <obo:RO_0001025 rdf:resource="http://purl.obolibrary.org/obo/GAZ_00014870"/>
        <obo:IAO_0000115>A sum (district) of Dornogovi Province in southeastern Mongolia.</obo:IAO_0000115>
        <oboInOwl:hasOBONamespace>GAZ</oboInOwl:hasOBONamespace>
        <oboInOwl:id>GAZ:00027158</oboInOwl:id>
        <rdfs:label>Airag District</rdfs:label>
    </owl:NamedIndividual>
    


    <!-- http://purl.obolibrary.org/obo/GAZ_00027159 -->

    <owl:NamedIndividual rdf:about="http://purl.obolibrary.org/obo/GAZ_00027159">
        <rdf:type rdf:resource="http://purl.obolibrary.org/obo/ENVO_00000004"/>
        <obo:RO_0001025 rdf:resource="http://purl.obolibrary.org/obo/GAZ_00014870"/>
        <obo:IAO_0000115>A sum (district) of Dornogovi Province in southeastern Mongolia.</obo:IAO_0000115>
        <oboInOwl:hasOBONamespace>GAZ</oboInOwl:hasOBONamespace>
        <oboInOwl:id>GAZ:00027159</oboInOwl:id>
        <rdfs:label>Mandakh District</rdfs:label>
    </owl:NamedIndividual>
    


    <!-- http://purl.obolibrary.org/obo/GAZ_00027160 -->

    <owl:NamedIndividual rdf:about="http://purl.obolibrary.org/obo/GAZ_00027160">
        <rdf:type rdf:resource="http://purl.obolibrary.org/obo/ENVO_00000004"/>
        <obo:RO_0001025 rdf:resource="http://purl.obolibrary.org/obo/GAZ_00014870"/>
        <obo:IAO_0000115>A sum (district) of Dornogovi Province in southeastern Mongolia.</obo:IAO_0000115>
        <oboInOwl:hasOBONamespace>GAZ</oboInOwl:hasOBONamespace>
        <oboInOwl:id>GAZ:00027160</oboInOwl:id>
        <rdfs:label>Dalanjargalan District</rdfs:label>
    </owl:NamedIndividual>
    


    <!-- http://purl.obolibrary.org/obo/GAZ_00027161 -->

    <owl:NamedIndividual rdf:about="http://purl.obolibrary.org/obo/GAZ_00027161">
        <rdf:type rdf:resource="http://purl.obolibrary.org/obo/ENVO_00000004"/>
        <obo:RO_0001025 rdf:resource="http://purl.obolibrary.org/obo/GAZ_00014870"/>
        <obo:IAO_0000115>A sum (district) of Dornogovi Province in southeastern Mongolia.</obo:IAO_0000115>
        <oboInOwl:hasOBONamespace>GAZ</oboInOwl:hasOBONamespace>
        <oboInOwl:id>GAZ:00027161</oboInOwl:id>
        <rdfs:label>Khatanbulag District</rdfs:label>
    </owl:NamedIndividual>
    


    <!-- http://purl.obolibrary.org/obo/GAZ_00027162 -->

    <owl:NamedIndividual rdf:about="http://purl.obolibrary.org/obo/GAZ_00027162">
        <rdf:type rdf:resource="http://purl.obolibrary.org/obo/ENVO_00000004"/>
        <obo:RO_0001025 rdf:resource="http://purl.obolibrary.org/obo/GAZ_00014870"/>
        <obo:IAO_0000115>A sum (district) of Dornogovi Province in southeastern Mongolia.</obo:IAO_0000115>
        <oboInOwl:hasOBONamespace>GAZ</oboInOwl:hasOBONamespace>
        <oboInOwl:id>GAZ:00027162</oboInOwl:id>
        <rdfs:label>Ikhkhet District</rdfs:label>
    </owl:NamedIndividual>
    


    <!-- http://purl.obolibrary.org/obo/GAZ_00027163 -->

    <owl:NamedIndividual rdf:about="http://purl.obolibrary.org/obo/GAZ_00027163">
        <rdf:type rdf:resource="http://purl.obolibrary.org/obo/ENVO_00000004"/>
        <obo:RO_0001025 rdf:resource="http://purl.obolibrary.org/obo/GAZ_00014870"/>
        <obo:IAO_0000115>A sum (district) of Dornogovi Province in southeastern Mongolia.</obo:IAO_0000115>
        <oboInOwl:hasOBONamespace>GAZ</oboInOwl:hasOBONamespace>
        <oboInOwl:id>GAZ:00027163</oboInOwl:id>
        <rdfs:label>Delgerekh District</rdfs:label>
    </owl:NamedIndividual>
    


    <!-- http://purl.obolibrary.org/obo/GAZ_00027164 -->

    <owl:NamedIndividual rdf:about="http://purl.obolibrary.org/obo/GAZ_00027164">
        <rdf:type rdf:resource="http://purl.obolibrary.org/obo/ENVO_00000004"/>
        <obo:RO_0001025 rdf:resource="http://purl.obolibrary.org/obo/GAZ_00014867"/>
        <obo:IAO_0000115>A sum (district) of Dundgovi Province in southern Mongolia.</obo:IAO_0000115>
        <oboInOwl:hasOBONamespace>GAZ</oboInOwl:hasOBONamespace>
        <oboInOwl:id>GAZ:00027164</oboInOwl:id>
        <rdfs:label>Ondorshil District</rdfs:label>
    </owl:NamedIndividual>
    


    <!-- http://purl.obolibrary.org/obo/GAZ_00027165 -->

    <owl:NamedIndividual rdf:about="http://purl.obolibrary.org/obo/GAZ_00027165">
        <rdf:type rdf:resource="http://purl.obolibrary.org/obo/ENVO_00000004"/>
        <obo:RO_0001025 rdf:resource="http://purl.obolibrary.org/obo/GAZ_00014867"/>
        <obo:IAO_0000115>A sum (district) of Dundgovi Province in southern Mongolia.</obo:IAO_0000115>
        <oboInOwl:hasOBONamespace>GAZ</oboInOwl:hasOBONamespace>
        <oboInOwl:id>GAZ:00027165</oboInOwl:id>
        <rdfs:label>Deren District</rdfs:label>
    </owl:NamedIndividual>
    


    <!-- http://purl.obolibrary.org/obo/GAZ_00027166 -->

    <owl:NamedIndividual rdf:about="http://purl.obolibrary.org/obo/GAZ_00027166">
        <rdf:type rdf:resource="http://purl.obolibrary.org/obo/ENVO_00000004"/>
        <obo:RO_0001025 rdf:resource="http://purl.obolibrary.org/obo/GAZ_00014867"/>
        <obo:IAO_0000115>A sum (district) of Dundgovi Province in southern Mongolia.</obo:IAO_0000115>
        <oboInOwl:hasOBONamespace>GAZ</oboInOwl:hasOBONamespace>
        <oboInOwl:id>GAZ:00027166</oboInOwl:id>
        <rdfs:label>Adaatsag District</rdfs:label>
    </owl:NamedIndividual>
    


    <!-- http://purl.obolibrary.org/obo/GAZ_00027167 -->

    <owl:NamedIndividual rdf:about="http://purl.obolibrary.org/obo/GAZ_00027167">
        <rdf:type rdf:resource="http://purl.obolibrary.org/obo/ENVO_00000004"/>
        <obo:RO_0001025 rdf:resource="http://purl.obolibrary.org/obo/GAZ_00014867"/>
        <obo:IAO_0000115>A sum (district) of Dundgovi Province in southern Mongolia.</obo:IAO_0000115>
        <oboInOwl:hasOBONamespace>GAZ</oboInOwl:hasOBONamespace>
        <oboInOwl:id>GAZ:00027167</oboInOwl:id>
        <rdfs:label>Erdenedalai District</rdfs:label>
    </owl:NamedIndividual>
    


    <!-- http://purl.obolibrary.org/obo/GAZ_00027168 -->

    <owl:NamedIndividual rdf:about="http://purl.obolibrary.org/obo/GAZ_00027168">
        <rdf:type rdf:resource="http://purl.obolibrary.org/obo/ENVO_00000004"/>
        <obo:RO_0001025 rdf:resource="http://purl.obolibrary.org/obo/GAZ_00014867"/>
        <obo:IAO_0000115>A sum (district) of Dundgovi Province in southern Mongolia.</obo:IAO_0000115>
        <oboInOwl:hasOBONamespace>GAZ</oboInOwl:hasOBONamespace>
        <oboInOwl:id>GAZ:00027168</oboInOwl:id>
        <rdfs:label>Delgerkhangai District</rdfs:label>
    </owl:NamedIndividual>
    


    <!-- http://purl.obolibrary.org/obo/GAZ_00027169 -->

    <owl:NamedIndividual rdf:about="http://purl.obolibrary.org/obo/GAZ_00027169">
        <rdf:type rdf:resource="http://purl.obolibrary.org/obo/ENVO_00000004"/>
        <obo:RO_0001025 rdf:resource="http://purl.obolibrary.org/obo/GAZ_00014867"/>
        <obo:IAO_0000115>A sum (district) of Dundgovi Province in southern Mongolia.</obo:IAO_0000115>
        <oboInOwl:hasOBONamespace>GAZ</oboInOwl:hasOBONamespace>
        <oboInOwl:id>GAZ:00027169</oboInOwl:id>
        <rdfs:label>Luus District</rdfs:label>
    </owl:NamedIndividual>
    


    <!-- http://purl.obolibrary.org/obo/GAZ_00027170 -->

    <owl:NamedIndividual rdf:about="http://purl.obolibrary.org/obo/GAZ_00027170">
        <rdf:type rdf:resource="http://purl.obolibrary.org/obo/ENVO_00000004"/>
        <obo:RO_0001025 rdf:resource="http://purl.obolibrary.org/obo/GAZ_00014867"/>
        <obo:IAO_0000115>A sum (district) of Dundgovi Province in southern Mongolia.</obo:IAO_0000115>
        <oboInOwl:hasOBONamespace>GAZ</oboInOwl:hasOBONamespace>
        <oboInOwl:id>GAZ:00027170</oboInOwl:id>
        <rdfs:label>Saikhan-Ovoo District</rdfs:label>
    </owl:NamedIndividual>
    


    <!-- http://purl.obolibrary.org/obo/GAZ_00027171 -->

    <owl:NamedIndividual rdf:about="http://purl.obolibrary.org/obo/GAZ_00027171">
        <rdf:type rdf:resource="http://purl.obolibrary.org/obo/ENVO_00000004"/>
        <obo:RO_0001025 rdf:resource="http://purl.obolibrary.org/obo/GAZ_00014867"/>
        <obo:IAO_0000115>A sum (district) of Dundgovi Province in southern Mongolia.</obo:IAO_0000115>
        <oboInOwl:hasOBONamespace>GAZ</oboInOwl:hasOBONamespace>
        <oboInOwl:id>GAZ:00027171</oboInOwl:id>
        <rdfs:label>Delgertsogt District</rdfs:label>
    </owl:NamedIndividual>
    


    <!-- http://purl.obolibrary.org/obo/GAZ_00027172 -->

    <owl:NamedIndividual rdf:about="http://purl.obolibrary.org/obo/GAZ_00027172">
        <rdf:type rdf:resource="http://purl.obolibrary.org/obo/ENVO_00000004"/>
        <obo:RO_0001025 rdf:resource="http://purl.obolibrary.org/obo/GAZ_00014867"/>
        <obo:IAO_0000115>A sum (district) of Dundgovi Province in southern Mongolia.</obo:IAO_0000115>
        <oboInOwl:hasOBONamespace>GAZ</oboInOwl:hasOBONamespace>
        <oboInOwl:id>GAZ:00027172</oboInOwl:id>
        <rdfs:label>Bayanjargalan District</rdfs:label>
    </owl:NamedIndividual>
    


    <!-- http://purl.obolibrary.org/obo/GAZ_00027173 -->

    <owl:NamedIndividual rdf:about="http://purl.obolibrary.org/obo/GAZ_00027173">
        <rdf:type rdf:resource="http://purl.obolibrary.org/obo/ENVO_00000004"/>
        <obo:RO_0001025 rdf:resource="http://purl.obolibrary.org/obo/GAZ_00014867"/>
        <obo:IAO_0000115>A sum (district) of Dundgovi Province in southern Mongolia.</obo:IAO_0000115>
        <oboInOwl:hasOBONamespace>GAZ</oboInOwl:hasOBONamespace>
        <oboInOwl:id>GAZ:00027173</oboInOwl:id>
        <rdfs:label>Gurvansaikhan District</rdfs:label>
    </owl:NamedIndividual>
    


    <!-- http://purl.obolibrary.org/obo/GAZ_00027174 -->

    <owl:NamedIndividual rdf:about="http://purl.obolibrary.org/obo/GAZ_00027174">
        <rdf:type rdf:resource="http://purl.obolibrary.org/obo/ENVO_00000004"/>
        <obo:RO_0001025 rdf:resource="http://purl.obolibrary.org/obo/GAZ_00014867"/>
        <obo:IAO_0000115>A sum (district) of Dundgovi Province in southern Mongolia.</obo:IAO_0000115>
        <oboInOwl:hasOBONamespace>GAZ</oboInOwl:hasOBONamespace>
        <oboInOwl:id>GAZ:00027174</oboInOwl:id>
        <rdfs:label>Govi-Ugtaal District</rdfs:label>
    </owl:NamedIndividual>
    


    <!-- http://purl.obolibrary.org/obo/GAZ_00027175 -->

    <owl:NamedIndividual rdf:about="http://purl.obolibrary.org/obo/GAZ_00027175">
        <rdf:type rdf:resource="http://purl.obolibrary.org/obo/ENVO_00000004"/>
        <obo:RO_0001025 rdf:resource="http://purl.obolibrary.org/obo/GAZ_00014867"/>
        <obo:IAO_0000115>A sum (district) of Dundgovi Province in southern Mongolia.</obo:IAO_0000115>
        <oboInOwl:hasOBONamespace>GAZ</oboInOwl:hasOBONamespace>
        <oboInOwl:id>GAZ:00027175</oboInOwl:id>
        <rdfs:label>Tsagaandelger District</rdfs:label>
    </owl:NamedIndividual>
    


    <!-- http://purl.obolibrary.org/obo/GAZ_00027176 -->

    <owl:NamedIndividual rdf:about="http://purl.obolibrary.org/obo/GAZ_00027176">
        <rdf:type rdf:resource="http://purl.obolibrary.org/obo/ENVO_00000004"/>
        <obo:RO_0001025 rdf:resource="http://purl.obolibrary.org/obo/GAZ_00014867"/>
        <obo:IAO_0000115>A sum (district) of Dundgovi Province in southern Mongolia.</obo:IAO_0000115>
        <oboInOwl:hasOBONamespace>GAZ</oboInOwl:hasOBONamespace>
        <oboInOwl:id>GAZ:00027176</oboInOwl:id>
        <rdfs:label>Khuld District</rdfs:label>
    </owl:NamedIndividual>
    


    <!-- http://purl.obolibrary.org/obo/GAZ_00027177 -->

    <owl:NamedIndividual rdf:about="http://purl.obolibrary.org/obo/GAZ_00027177">
        <rdf:type rdf:resource="http://purl.obolibrary.org/obo/ENVO_00000004"/>
        <obo:RO_0001025 rdf:resource="http://purl.obolibrary.org/obo/GAZ_00014867"/>
        <obo:IAO_0000115>A sum (district) of Dundgovi Province in southern Mongolia.</obo:IAO_0000115>
        <oboInOwl:hasOBONamespace>GAZ</oboInOwl:hasOBONamespace>
        <oboInOwl:id>GAZ:00027177</oboInOwl:id>
        <rdfs:label>Olziit District</rdfs:label>
    </owl:NamedIndividual>
    


    <!-- http://purl.obolibrary.org/obo/GAZ_00027178 -->

    <owl:NamedIndividual rdf:about="http://purl.obolibrary.org/obo/GAZ_00027178">
        <rdf:type rdf:resource="http://purl.obolibrary.org/obo/ENVO_00000004"/>
        <obo:RO_0001025 rdf:resource="http://purl.obolibrary.org/obo/GAZ_00014867"/>
        <obo:IAO_0000115>A sum (district) of Dundgovi Province in southern Mongolia.</obo:IAO_0000115>
        <oboInOwl:hasOBONamespace>GAZ</oboInOwl:hasOBONamespace>
        <oboInOwl:id>GAZ:00027178</oboInOwl:id>
        <rdfs:label>Saintsagaan District</rdfs:label>
    </owl:NamedIndividual>
    


    <!-- http://purl.obolibrary.org/obo/GAZ_00027179 -->

    <owl:NamedIndividual rdf:about="http://purl.obolibrary.org/obo/GAZ_00027179">
        <rdf:type rdf:resource="http://purl.obolibrary.org/obo/ENVO_00000004"/>
        <obo:RO_0001025 rdf:resource="http://purl.obolibrary.org/obo/GAZ_00014873"/>
        <obo:IAO_0000115>A sum (district) of Khentii Province in eastern Mongolia.</obo:IAO_0000115>
        <oboInOwl:hasOBONamespace>GAZ</oboInOwl:hasOBONamespace>
        <oboInOwl:id>GAZ:00027179</oboInOwl:id>
        <rdfs:label>Norovlin District</rdfs:label>
    </owl:NamedIndividual>
    


    <!-- http://purl.obolibrary.org/obo/GAZ_00027180 -->

    <owl:NamedIndividual rdf:about="http://purl.obolibrary.org/obo/GAZ_00027180">
        <rdf:type rdf:resource="http://purl.obolibrary.org/obo/ENVO_00000004"/>
        <obo:RO_0001025 rdf:resource="http://purl.obolibrary.org/obo/GAZ_00014873"/>
        <obo:IAO_0000115>A sum (district) of Khentii Province in eastern Mongolia.</obo:IAO_0000115>
        <oboInOwl:hasOBONamespace>GAZ</oboInOwl:hasOBONamespace>
        <oboInOwl:id>GAZ:00027180</oboInOwl:id>
        <rdfs:label>Darkhan District</rdfs:label>
    </owl:NamedIndividual>
    


    <!-- http://purl.obolibrary.org/obo/GAZ_00027181 -->

    <owl:NamedIndividual rdf:about="http://purl.obolibrary.org/obo/GAZ_00027181">
        <rdf:type rdf:resource="http://purl.obolibrary.org/obo/ENVO_00000004"/>
        <obo:RO_0001025 rdf:resource="http://purl.obolibrary.org/obo/GAZ_00014879"/>
        <obo:IAO_0000115>A sum (district) of Govi-Altai Aimag (province) in western Mongolia.</obo:IAO_0000115>
        <oboInOwl:hasOBONamespace>GAZ</oboInOwl:hasOBONamespace>
        <oboInOwl:id>GAZ:00027181</oboInOwl:id>
        <rdfs:label>Altai District</rdfs:label>
    </owl:NamedIndividual>
    


    <!-- http://purl.obolibrary.org/obo/GAZ_00027182 -->

    <owl:NamedIndividual rdf:about="http://purl.obolibrary.org/obo/GAZ_00027182">
        <rdf:type rdf:resource="http://purl.obolibrary.org/obo/ENVO_00000004"/>
        <obo:RO_0001025 rdf:resource="http://purl.obolibrary.org/obo/GAZ_00014873"/>
        <obo:IAO_0000115>A sum (district) of Khentii Province in eastern Mongolia.</obo:IAO_0000115>
        <oboInOwl:hasOBONamespace>GAZ</oboInOwl:hasOBONamespace>
        <oboInOwl:id>GAZ:00027182</oboInOwl:id>
        <rdfs:label>Bayan-Adarga District</rdfs:label>
    </owl:NamedIndividual>
    


    <!-- http://purl.obolibrary.org/obo/GAZ_00027183 -->

    <owl:NamedIndividual rdf:about="http://purl.obolibrary.org/obo/GAZ_00027183">
        <rdf:type rdf:resource="http://purl.obolibrary.org/obo/ENVO_00000004"/>
        <obo:RO_0001025 rdf:resource="http://purl.obolibrary.org/obo/GAZ_00014873"/>
        <obo:IAO_0000115>A sum (district) of Khentii Province in eastern Mongolia.</obo:IAO_0000115>
        <oboInOwl:hasOBONamespace>GAZ</oboInOwl:hasOBONamespace>
        <oboInOwl:id>GAZ:00027183</oboInOwl:id>
        <rdfs:label>Bayan-Ovoo District</rdfs:label>
    </owl:NamedIndividual>
    


    <!-- http://purl.obolibrary.org/obo/GAZ_00027184 -->

    <owl:NamedIndividual rdf:about="http://purl.obolibrary.org/obo/GAZ_00027184">
        <obo:RO_0001025 rdf:resource="http://purl.obolibrary.org/obo/GAZ_00027180"/>
        <obo:IAO_0000115>A populated place. A city in Khentii Province in eastern Mongolia. Bor-Ondor is situated in Darkhan sum (district), but is administrated separately.</obo:IAO_0000115>
        <oboInOwl:hasOBONamespace>GAZ</oboInOwl:hasOBONamespace>
        <oboInOwl:id>GAZ:00027184</oboInOwl:id>
        <rdfs:label>Bor-Ondor City</rdfs:label>
    </owl:NamedIndividual>
    


    <!-- http://purl.obolibrary.org/obo/GAZ_00027185 -->

    <owl:NamedIndividual rdf:about="http://purl.obolibrary.org/obo/GAZ_00027185">
        <rdf:type rdf:resource="http://purl.obolibrary.org/obo/ENVO_00000004"/>
        <obo:RO_0001025 rdf:resource="http://purl.obolibrary.org/obo/GAZ_00014873"/>
        <obo:IAO_0000115>A sum (district) of Khentii Province in eastern Mongolia.</obo:IAO_0000115>
        <oboInOwl:hasOBONamespace>GAZ</oboInOwl:hasOBONamespace>
        <oboInOwl:id>GAZ:00027185</oboInOwl:id>
        <rdfs:label>Tsenkhermandal District</rdfs:label>
    </owl:NamedIndividual>
    


    <!-- http://purl.obolibrary.org/obo/GAZ_00027186 -->

    <owl:NamedIndividual rdf:about="http://purl.obolibrary.org/obo/GAZ_00027186">
        <obo:RO_0001025 rdf:resource="http://purl.obolibrary.org/obo/GAZ_00014871"/>
        <obo:IAO_0000115>A sum of Govisumber Province in central Mongolia.</obo:IAO_0000115>
        <oboInOwl:hasOBONamespace>GAZ</oboInOwl:hasOBONamespace>
        <oboInOwl:id>GAZ:00027186</oboInOwl:id>
        <rdfs:label>Bayantal District</rdfs:label>
    </owl:NamedIndividual>
    


    <!-- http://purl.obolibrary.org/obo/GAZ_00027187 -->

    <owl:NamedIndividual rdf:about="http://purl.obolibrary.org/obo/GAZ_00027187">
        <rdf:type rdf:resource="http://purl.obolibrary.org/obo/ENVO_00000004"/>
        <obo:RO_0001025 rdf:resource="http://purl.obolibrary.org/obo/GAZ_00014873"/>
        <obo:IAO_0000115>A sum (district) of Khentii Province in eastern Mongolia.</obo:IAO_0000115>
        <oboInOwl:hasOBONamespace>GAZ</oboInOwl:hasOBONamespace>
        <oboInOwl:id>GAZ:00027187</oboInOwl:id>
        <rdfs:label>Moron District</rdfs:label>
    </owl:NamedIndividual>
    


    <!-- http://purl.obolibrary.org/obo/GAZ_00027188 -->

    <owl:NamedIndividual rdf:about="http://purl.obolibrary.org/obo/GAZ_00027188">
        <rdf:type rdf:resource="http://purl.obolibrary.org/obo/ENVO_00000856"/>
        <obo:RO_0001025 rdf:resource="http://purl.obolibrary.org/obo/GAZ_00027191"/>
        <obo:IAO_0000115>A populated place. A town in the Batnorov sum (district) of Khentii Province in eastern Mongolia.</obo:IAO_0000115>
        <oboInOwl:hasOBONamespace>GAZ</oboInOwl:hasOBONamespace>
        <oboInOwl:id>GAZ:00027188</oboInOwl:id>
        <rdfs:label>Berkh City</rdfs:label>
    </owl:NamedIndividual>
    


    <!-- http://purl.obolibrary.org/obo/GAZ_00027189 -->

    <owl:NamedIndividual rdf:about="http://purl.obolibrary.org/obo/GAZ_00027189">
        <rdf:type rdf:resource="http://purl.obolibrary.org/obo/ENVO_00000004"/>
        <obo:RO_0001025 rdf:resource="http://purl.obolibrary.org/obo/GAZ_00014873"/>
        <obo:IAO_0000115>A sum (district) of Khentii Province in eastern Mongolia.</obo:IAO_0000115>
        <oboInOwl:hasOBONamespace>GAZ</oboInOwl:hasOBONamespace>
        <oboInOwl:id>GAZ:00027189</oboInOwl:id>
        <rdfs:label>Omnodelger District</rdfs:label>
    </owl:NamedIndividual>
    


    <!-- http://purl.obolibrary.org/obo/GAZ_00027190 -->

    <owl:NamedIndividual rdf:about="http://purl.obolibrary.org/obo/GAZ_00027190">
        <rdf:type rdf:resource="http://purl.obolibrary.org/obo/ENVO_00000004"/>
        <obo:RO_0001025 rdf:resource="http://purl.obolibrary.org/obo/GAZ_00014879"/>
        <obo:IAO_0000115>A sum (district) of Govi-Altai Aimag (province) in western Mongolia.</obo:IAO_0000115>
        <oboInOwl:hasOBONamespace>GAZ</oboInOwl:hasOBONamespace>
        <oboInOwl:id>GAZ:00027190</oboInOwl:id>
        <rdfs:label>Togrog District</rdfs:label>
    </owl:NamedIndividual>
    


    <!-- http://purl.obolibrary.org/obo/GAZ_00027191 -->

    <owl:NamedIndividual rdf:about="http://purl.obolibrary.org/obo/GAZ_00027191">
        <rdf:type rdf:resource="http://purl.obolibrary.org/obo/ENVO_00000004"/>
        <obo:RO_0001025 rdf:resource="http://purl.obolibrary.org/obo/GAZ_00014873"/>
        <obo:IAO_0000115>A sum (district) of Khentii Province in eastern Mongolia.</obo:IAO_0000115>
        <oboInOwl:hasOBONamespace>GAZ</oboInOwl:hasOBONamespace>
        <oboInOwl:id>GAZ:00027191</oboInOwl:id>
        <rdfs:label>Batnorov District</rdfs:label>
    </owl:NamedIndividual>
    


    <!-- http://purl.obolibrary.org/obo/GAZ_00027192 -->

    <owl:NamedIndividual rdf:about="http://purl.obolibrary.org/obo/GAZ_00027192">
        <rdf:type rdf:resource="http://purl.obolibrary.org/obo/ENVO_00000856"/>
        <obo:RO_0001025 rdf:resource="http://purl.obolibrary.org/obo/GAZ_00027219"/>
        <obo:IAO_0000115>A populated place. A town in Mongolia located 290 km east of Ulan Bator. It is the capital of the Khentii Aimag (province).</obo:IAO_0000115>
        <oboInOwl:hasOBONamespace>GAZ</oboInOwl:hasOBONamespace>
        <oboInOwl:id>GAZ:00027192</oboInOwl:id>
        <rdfs:label>Ondorkhaan City</rdfs:label>
    </owl:NamedIndividual>
    


    <!-- http://purl.obolibrary.org/obo/GAZ_00027193 -->

    <owl:NamedIndividual rdf:about="http://purl.obolibrary.org/obo/GAZ_00027193">
        <rdf:type rdf:resource="http://purl.obolibrary.org/obo/ENVO_00000004"/>
        <obo:RO_0001025 rdf:resource="http://purl.obolibrary.org/obo/GAZ_00014873"/>
        <obo:IAO_0000115>A sum (district) of Khentii Province in eastern Mongolia.</obo:IAO_0000115>
        <oboInOwl:hasOBONamespace>GAZ</oboInOwl:hasOBONamespace>
        <oboInOwl:id>GAZ:00027193</oboInOwl:id>
        <rdfs:label>Dadal District</rdfs:label>
    </owl:NamedIndividual>
    


    <!-- http://purl.obolibrary.org/obo/GAZ_00027194 -->

    <owl:NamedIndividual rdf:about="http://purl.obolibrary.org/obo/GAZ_00027194">
        <rdf:type rdf:resource="http://purl.obolibrary.org/obo/ENVO_00000004"/>
        <obo:RO_0001025 rdf:resource="http://purl.obolibrary.org/obo/GAZ_00014873"/>
        <obo:IAO_0000115>A sum (district) of Khentii Province in eastern Mongolia.</obo:IAO_0000115>
        <oboInOwl:hasOBONamespace>GAZ</oboInOwl:hasOBONamespace>
        <oboInOwl:id>GAZ:00027194</oboInOwl:id>
        <rdfs:label>Galshar District</rdfs:label>
    </owl:NamedIndividual>
    


    <!-- http://purl.obolibrary.org/obo/GAZ_00027195 -->

    <owl:NamedIndividual rdf:about="http://purl.obolibrary.org/obo/GAZ_00027195">
        <rdf:type rdf:resource="http://purl.obolibrary.org/obo/ENVO_00000004"/>
        <obo:RO_0001025 rdf:resource="http://purl.obolibrary.org/obo/GAZ_00014879"/>
        <obo:IAO_0000115>A sum (district) of Govi-Altai Aimag (province) in western Mongolia.</obo:IAO_0000115>
        <oboInOwl:hasOBONamespace>GAZ</oboInOwl:hasOBONamespace>
        <oboInOwl:id>GAZ:00027195</oboInOwl:id>
        <rdfs:label>Khokh morit District</rdfs:label>
    </owl:NamedIndividual>
    


    <!-- http://purl.obolibrary.org/obo/GAZ_00027196 -->

    <owl:NamedIndividual rdf:about="http://purl.obolibrary.org/obo/GAZ_00027196">
        <rdf:type rdf:resource="http://purl.obolibrary.org/obo/ENVO_00000004"/>
        <obo:RO_0001025 rdf:resource="http://purl.obolibrary.org/obo/GAZ_00014879"/>
        <obo:IAO_0000115>A sum (district) of Govi-Altai Aimag (province) in western Mongolia.</obo:IAO_0000115>
        <oboInOwl:hasOBONamespace>GAZ</oboInOwl:hasOBONamespace>
        <oboInOwl:id>GAZ:00027196</oboInOwl:id>
        <rdfs:label>Delger District</rdfs:label>
    </owl:NamedIndividual>
    


    <!-- http://purl.obolibrary.org/obo/GAZ_00027197 -->

    <owl:NamedIndividual rdf:about="http://purl.obolibrary.org/obo/GAZ_00027197">
        <rdf:type rdf:resource="http://purl.obolibrary.org/obo/ENVO_00000004"/>
        <obo:RO_0001025 rdf:resource="http://purl.obolibrary.org/obo/GAZ_00014879"/>
        <obo:IAO_0000115>A sum (district) of Govi-Altai Aimag (province) in western Mongolia.</obo:IAO_0000115>
        <oboInOwl:hasOBONamespace>GAZ</oboInOwl:hasOBONamespace>
        <oboInOwl:id>GAZ:00027197</oboInOwl:id>
        <rdfs:label>Tsogt District</rdfs:label>
    </owl:NamedIndividual>
    


    <!-- http://purl.obolibrary.org/obo/GAZ_00027198 -->

    <owl:NamedIndividual rdf:about="http://purl.obolibrary.org/obo/GAZ_00027198">
        <rdf:type rdf:resource="http://purl.obolibrary.org/obo/ENVO_00000004"/>
        <obo:RO_0001025 rdf:resource="http://purl.obolibrary.org/obo/GAZ_00014879"/>
        <obo:IAO_0000115>A sum (district) of Govi-Altai Aimag (province) in western Mongolia.</obo:IAO_0000115>
        <oboInOwl:hasOBONamespace>GAZ</oboInOwl:hasOBONamespace>
        <oboInOwl:id>GAZ:00027198</oboInOwl:id>
        <rdfs:label>Chandmani District</rdfs:label>
    </owl:NamedIndividual>
    


    <!-- http://purl.obolibrary.org/obo/GAZ_00027199 -->

    <owl:NamedIndividual rdf:about="http://purl.obolibrary.org/obo/GAZ_00027199">
        <rdf:type rdf:resource="http://purl.obolibrary.org/obo/ENVO_00000004"/>
        <obo:RO_0001025 rdf:resource="http://purl.obolibrary.org/obo/GAZ_00014879"/>
        <obo:IAO_0000115>A sum (district) of Govi-Altai Aimag (province) in western Mongolia.</obo:IAO_0000115>
        <oboInOwl:hasOBONamespace>GAZ</oboInOwl:hasOBONamespace>
        <oboInOwl:id>GAZ:00027199</oboInOwl:id>
        <rdfs:label>Biger District</rdfs:label>
    </owl:NamedIndividual>
    


    <!-- http://purl.obolibrary.org/obo/GAZ_00027200 -->

    <owl:NamedIndividual rdf:about="http://purl.obolibrary.org/obo/GAZ_00027200">
        <rdf:type rdf:resource="http://purl.obolibrary.org/obo/ENVO_00000004"/>
        <obo:RO_0001025 rdf:resource="http://purl.obolibrary.org/obo/GAZ_00014879"/>
        <obo:IAO_0000115>A sum (district) of Govi-Altai Aimag (province) in western Mongolia.</obo:IAO_0000115>
        <oboInOwl:hasOBONamespace>GAZ</oboInOwl:hasOBONamespace>
        <oboInOwl:id>GAZ:00027200</oboInOwl:id>
        <rdfs:label>Sharga District</rdfs:label>
    </owl:NamedIndividual>
    


    <!-- http://purl.obolibrary.org/obo/GAZ_00027201 -->

    <owl:NamedIndividual rdf:about="http://purl.obolibrary.org/obo/GAZ_00027201">
        <rdf:type rdf:resource="http://purl.obolibrary.org/obo/ENVO_00000004"/>
        <obo:RO_0001025 rdf:resource="http://purl.obolibrary.org/obo/GAZ_00014879"/>
        <obo:IAO_0000115>A sum (district) of Govi-Altai Aimag (province) in western Mongolia.</obo:IAO_0000115>
        <oboInOwl:hasOBONamespace>GAZ</oboInOwl:hasOBONamespace>
        <oboInOwl:id>GAZ:00027201</oboInOwl:id>
        <rdfs:label>Khaliun District</rdfs:label>
    </owl:NamedIndividual>
    


    <!-- http://purl.obolibrary.org/obo/GAZ_00027202 -->

    <owl:NamedIndividual rdf:about="http://purl.obolibrary.org/obo/GAZ_00027202">
        <rdf:type rdf:resource="http://purl.obolibrary.org/obo/ENVO_00000004"/>
        <obo:RO_0001025 rdf:resource="http://purl.obolibrary.org/obo/GAZ_00014873"/>
        <obo:IAO_0000115>A sum (district) of Khentii Province in eastern Mongolia.</obo:IAO_0000115>
        <oboInOwl:hasOBONamespace>GAZ</oboInOwl:hasOBONamespace>
        <oboInOwl:id>GAZ:00027202</oboInOwl:id>
        <rdfs:label>Batshireet District</rdfs:label>
    </owl:NamedIndividual>
    


    <!-- http://purl.obolibrary.org/obo/GAZ_00027203 -->

    <owl:NamedIndividual rdf:about="http://purl.obolibrary.org/obo/GAZ_00027203">
        <rdf:type rdf:resource="http://purl.obolibrary.org/obo/ENVO_00000004"/>
        <obo:RO_0001025 rdf:resource="http://purl.obolibrary.org/obo/GAZ_00014879"/>
        <obo:IAO_0000115>A sum (district) of Govi-Altai Aimag (province) in western Mongolia.</obo:IAO_0000115>
        <oboInOwl:hasOBONamespace>GAZ</oboInOwl:hasOBONamespace>
        <oboInOwl:id>GAZ:00027203</oboInOwl:id>
        <rdfs:label>Darvi District</rdfs:label>
    </owl:NamedIndividual>
    


    <!-- http://purl.obolibrary.org/obo/GAZ_00027204 -->

    <owl:NamedIndividual rdf:about="http://purl.obolibrary.org/obo/GAZ_00027204">
        <rdf:type rdf:resource="http://purl.obolibrary.org/obo/ENVO_00000004"/>
        <obo:RO_0001025 rdf:resource="http://purl.obolibrary.org/obo/GAZ_00014879"/>
        <obo:IAO_0000115>A sum (district) of Govi-Altai Aimag (province) in western Mongolia.</obo:IAO_0000115>
        <oboInOwl:hasOBONamespace>GAZ</oboInOwl:hasOBONamespace>
        <oboInOwl:id>GAZ:00027204</oboInOwl:id>
        <rdfs:label>Tseel District</rdfs:label>
    </owl:NamedIndividual>
    


    <!-- http://purl.obolibrary.org/obo/GAZ_00027205 -->

    <owl:NamedIndividual rdf:about="http://purl.obolibrary.org/obo/GAZ_00027205">
        <obo:RO_0001025 rdf:resource="http://purl.obolibrary.org/obo/GAZ_00014871"/>
        <obo:IAO_0000115>A sum of Govisumber Province in central Mongolia.</obo:IAO_0000115>
        <oboInOwl:hasOBONamespace>GAZ</oboInOwl:hasOBONamespace>
        <oboInOwl:id>GAZ:00027205</oboInOwl:id>
        <rdfs:label>Shiveegovi District</rdfs:label>
    </owl:NamedIndividual>
    


    <!-- http://purl.obolibrary.org/obo/GAZ_00027206 -->

    <owl:NamedIndividual rdf:about="http://purl.obolibrary.org/obo/GAZ_00027206">
        <rdf:type rdf:resource="http://purl.obolibrary.org/obo/ENVO_00000004"/>
        <obo:RO_0001025 rdf:resource="http://purl.obolibrary.org/obo/GAZ_00014873"/>
        <obo:IAO_0000115>A sum (district) of Khentii Province in eastern Mongolia.</obo:IAO_0000115>
        <oboInOwl:hasOBONamespace>GAZ</oboInOwl:hasOBONamespace>
        <oboInOwl:id>GAZ:00027206</oboInOwl:id>
        <rdfs:label>Bayankhutag District</rdfs:label>
    </owl:NamedIndividual>
    


    <!-- http://purl.obolibrary.org/obo/GAZ_00027207 -->

    <owl:NamedIndividual rdf:about="http://purl.obolibrary.org/obo/GAZ_00027207">
        <rdf:type rdf:resource="http://purl.obolibrary.org/obo/ENVO_00000004"/>
        <obo:RO_0001025 rdf:resource="http://purl.obolibrary.org/obo/GAZ_00014879"/>
        <obo:IAO_0000115>A sum (district) of Govi-Altai Aimag (province) in western Mongolia.</obo:IAO_0000115>
        <oboInOwl:hasOBONamespace>GAZ</oboInOwl:hasOBONamespace>
        <oboInOwl:id>GAZ:00027207</oboInOwl:id>
        <rdfs:label>Erdene District</rdfs:label>
    </owl:NamedIndividual>
    


    <!-- http://purl.obolibrary.org/obo/GAZ_00027208 -->

    <owl:NamedIndividual rdf:about="http://purl.obolibrary.org/obo/GAZ_00027208">
        <rdf:type rdf:resource="http://purl.obolibrary.org/obo/ENVO_00000004"/>
        <obo:RO_0001025 rdf:resource="http://purl.obolibrary.org/obo/GAZ_00014879"/>
        <obo:IAO_0000115>A sum (district) of Govi-Altai Aimag (province) in western Mongolia.</obo:IAO_0000115>
        <oboInOwl:hasOBONamespace>GAZ</oboInOwl:hasOBONamespace>
        <oboInOwl:id>GAZ:00027208</oboInOwl:id>
        <rdfs:label>Taishir District</rdfs:label>
    </owl:NamedIndividual>
    


    <!-- http://purl.obolibrary.org/obo/GAZ_00027209 -->

    <owl:NamedIndividual rdf:about="http://purl.obolibrary.org/obo/GAZ_00027209">
        <rdf:type rdf:resource="http://purl.obolibrary.org/obo/ENVO_00000004"/>
        <obo:RO_0001025 rdf:resource="http://purl.obolibrary.org/obo/GAZ_00014879"/>
        <obo:IAO_0000115>A sum (district) of Govi-Altai Aimag (province) in western Mongolia.</obo:IAO_0000115>
        <oboInOwl:hasOBONamespace>GAZ</oboInOwl:hasOBONamespace>
        <oboInOwl:id>GAZ:00027209</oboInOwl:id>
        <rdfs:label>Bayan-Uul District</rdfs:label>
    </owl:NamedIndividual>
    


    <!-- http://purl.obolibrary.org/obo/GAZ_00027210 -->

    <owl:NamedIndividual rdf:about="http://purl.obolibrary.org/obo/GAZ_00027210">
        <rdf:type rdf:resource="http://purl.obolibrary.org/obo/ENVO_00000004"/>
        <obo:RO_0001025 rdf:resource="http://purl.obolibrary.org/obo/GAZ_00014879"/>
        <obo:IAO_0000115>A sum (district) of Govi-Altai Aimag (province) in western Mongolia.</obo:IAO_0000115>
        <oboInOwl:hasOBONamespace>GAZ</oboInOwl:hasOBONamespace>
        <oboInOwl:id>GAZ:00027210</oboInOwl:id>
        <rdfs:label>Jargalan District</rdfs:label>
    </owl:NamedIndividual>
    


    <!-- http://purl.obolibrary.org/obo/GAZ_00027211 -->

    <owl:NamedIndividual rdf:about="http://purl.obolibrary.org/obo/GAZ_00027211">
        <rdf:type rdf:resource="http://purl.obolibrary.org/obo/ENVO_00000004"/>
        <obo:RO_0001025 rdf:resource="http://purl.obolibrary.org/obo/GAZ_00014879"/>
        <obo:IAO_0000115>A sum (district) of Govi-Altai Aimag (province) in western Mongolia.</obo:IAO_0000115>
        <oboInOwl:hasOBONamespace>GAZ</oboInOwl:hasOBONamespace>
        <oboInOwl:id>GAZ:00027211</oboInOwl:id>
        <rdfs:label>Bugat District</rdfs:label>
    </owl:NamedIndividual>
    


    <!-- http://purl.obolibrary.org/obo/GAZ_00027212 -->

    <owl:NamedIndividual rdf:about="http://purl.obolibrary.org/obo/GAZ_00027212">
        <rdf:type rdf:resource="http://purl.obolibrary.org/obo/ENVO_00000004"/>
        <obo:RO_0001025 rdf:resource="http://purl.obolibrary.org/obo/GAZ_00014873"/>
        <obo:IAO_0000115>A sum (district) of Khentii Province in eastern Mongolia.</obo:IAO_0000115>
        <oboInOwl:hasOBONamespace>GAZ</oboInOwl:hasOBONamespace>
        <oboInOwl:id>GAZ:00027212</oboInOwl:id>
        <rdfs:label>Binder District</rdfs:label>
    </owl:NamedIndividual>
    


    <!-- http://purl.obolibrary.org/obo/GAZ_00027213 -->

    <owl:NamedIndividual rdf:about="http://purl.obolibrary.org/obo/GAZ_00027213">
        <obo:RO_0001025 rdf:resource="http://purl.obolibrary.org/obo/GAZ_00014871"/>
        <obo:IAO_0000115>A sum of Govisumber Province in central Mongolia.</obo:IAO_0000115>
        <oboInOwl:hasOBONamespace>GAZ</oboInOwl:hasOBONamespace>
        <oboInOwl:id>GAZ:00027213</oboInOwl:id>
        <rdfs:label>Sumber District</rdfs:label>
    </owl:NamedIndividual>
    


    <!-- http://purl.obolibrary.org/obo/GAZ_00027214 -->

    <owl:NamedIndividual rdf:about="http://purl.obolibrary.org/obo/GAZ_00027214">
        <rdf:type rdf:resource="http://purl.obolibrary.org/obo/ENVO_00000004"/>
        <obo:RO_0001025 rdf:resource="http://purl.obolibrary.org/obo/GAZ_00014873"/>
        <obo:IAO_0000115>A sum (district) of Khentii Province in eastern Mongolia.</obo:IAO_0000115>
        <oboInOwl:hasOBONamespace>GAZ</oboInOwl:hasOBONamespace>
        <oboInOwl:id>GAZ:00027214</oboInOwl:id>
        <rdfs:label>Bayanmonkh District</rdfs:label>
    </owl:NamedIndividual>
    


    <!-- http://purl.obolibrary.org/obo/GAZ_00027215 -->

    <owl:NamedIndividual rdf:about="http://purl.obolibrary.org/obo/GAZ_00027215">
        <rdf:type rdf:resource="http://purl.obolibrary.org/obo/ENVO_00000004"/>
        <obo:RO_0001025 rdf:resource="http://purl.obolibrary.org/obo/GAZ_00014873"/>
        <obo:IAO_0000115>A sum (district) of Khentii Province in eastern Mongolia.</obo:IAO_0000115>
        <oboInOwl:hasOBONamespace>GAZ</oboInOwl:hasOBONamespace>
        <oboInOwl:id>GAZ:00027215</oboInOwl:id>
        <rdfs:label>Delgerkhaan District</rdfs:label>
    </owl:NamedIndividual>
    


    <!-- http://purl.obolibrary.org/obo/GAZ_00027216 -->

    <owl:NamedIndividual rdf:about="http://purl.obolibrary.org/obo/GAZ_00027216">
        <rdf:type rdf:resource="http://purl.obolibrary.org/obo/ENVO_00000004"/>
        <obo:RO_0001025 rdf:resource="http://purl.obolibrary.org/obo/GAZ_00014879"/>
        <obo:IAO_0000115>A sum (district) of Govi-Altai Aimag (province) in western Mongolia.</obo:IAO_0000115>
        <oboInOwl:hasOBONamespace>GAZ</oboInOwl:hasOBONamespace>
        <oboInOwl:id>GAZ:00027216</oboInOwl:id>
        <rdfs:label>Yesonbulag District</rdfs:label>
    </owl:NamedIndividual>
    


    <!-- http://purl.obolibrary.org/obo/GAZ_00027217 -->

    <owl:NamedIndividual rdf:about="http://purl.obolibrary.org/obo/GAZ_00027217">
        <rdf:type rdf:resource="http://purl.obolibrary.org/obo/ENVO_00000004"/>
        <obo:RO_0001025 rdf:resource="http://purl.obolibrary.org/obo/GAZ_00014879"/>
        <obo:IAO_0000115>A sum (district) of Govi-Altai Aimag (province) in western Mongolia.</obo:IAO_0000115>
        <oboInOwl:hasOBONamespace>GAZ</oboInOwl:hasOBONamespace>
        <oboInOwl:id>GAZ:00027217</oboInOwl:id>
        <rdfs:label>Tonkhil District</rdfs:label>
    </owl:NamedIndividual>
    


    <!-- http://purl.obolibrary.org/obo/GAZ_00027218 -->

    <owl:NamedIndividual rdf:about="http://purl.obolibrary.org/obo/GAZ_00027218">
        <rdf:type rdf:resource="http://purl.obolibrary.org/obo/ENVO_00000004"/>
        <obo:RO_0001025 rdf:resource="http://purl.obolibrary.org/obo/GAZ_00014873"/>
        <obo:IAO_0000115>A sum (district) of Khentii Province in eastern Mongolia.</obo:IAO_0000115>
        <oboInOwl:hasOBONamespace>GAZ</oboInOwl:hasOBONamespace>
        <oboInOwl:id>GAZ:00027218</oboInOwl:id>
        <rdfs:label>Jargaltkhaan District</rdfs:label>
    </owl:NamedIndividual>
    


    <!-- http://purl.obolibrary.org/obo/GAZ_00027219 -->

    <owl:NamedIndividual rdf:about="http://purl.obolibrary.org/obo/GAZ_00027219">
        <rdf:type rdf:resource="http://purl.obolibrary.org/obo/ENVO_00000004"/>
        <obo:RO_0001025 rdf:resource="http://purl.obolibrary.org/obo/GAZ_00014873"/>
        <obo:IAO_0000115>A sum (district) of Khentii Province in eastern Mongolia.</obo:IAO_0000115>
        <oboInOwl:hasOBONamespace>GAZ</oboInOwl:hasOBONamespace>
        <oboInOwl:id>GAZ:00027219</oboInOwl:id>
        <rdfs:label>Kherlen District</rdfs:label>
    </owl:NamedIndividual>
    


    <!-- http://purl.obolibrary.org/obo/GAZ_00027220 -->

    <owl:NamedIndividual rdf:about="http://purl.obolibrary.org/obo/GAZ_00027220">
        <obo:RO_0001025 rdf:resource="http://purl.obolibrary.org/obo/GAZ_00014885"/>
        <obo:IAO_0000115>A sum of Khovsgol aimag.</obo:IAO_0000115>
        <oboInOwl:hasOBONamespace>GAZ</oboInOwl:hasOBONamespace>
        <oboInOwl:id>GAZ:00027220</oboInOwl:id>
        <rdfs:label>Khankh District</rdfs:label>
    </owl:NamedIndividual>
    


    <!-- http://purl.obolibrary.org/obo/GAZ_00027221 -->

    <owl:NamedIndividual rdf:about="http://purl.obolibrary.org/obo/GAZ_00027221">
        <obo:RO_0001025 rdf:resource="http://purl.obolibrary.org/obo/GAZ_00014885"/>
        <obo:IAO_0000115>A sum of Khovsgol aimag. In 1955, Rashaant sum was united with Tarialan, but became separate again in 1959.</obo:IAO_0000115>
        <oboInOwl:hasOBONamespace>GAZ</oboInOwl:hasOBONamespace>
        <oboInOwl:id>GAZ:00027221</oboInOwl:id>
        <rdfs:label>Rashaant District</rdfs:label>
    </owl:NamedIndividual>
    


    <!-- http://purl.obolibrary.org/obo/GAZ_00027222 -->

    <owl:NamedIndividual rdf:about="http://purl.obolibrary.org/obo/GAZ_00027222">
        <rdf:type rdf:resource="http://purl.obolibrary.org/obo/ENVO_00000004"/>
        <obo:RO_0001025 rdf:resource="http://purl.obolibrary.org/obo/GAZ_00014883"/>
        <obo:IAO_0000115>A sum (district) of Khovd Province in western Mongolia.</obo:IAO_0000115>
        <oboInOwl:hasOBONamespace>GAZ</oboInOwl:hasOBONamespace>
        <oboInOwl:id>GAZ:00027222</oboInOwl:id>
        <rdfs:label>Altai District</rdfs:label>
    </owl:NamedIndividual>
    


    <!-- http://purl.obolibrary.org/obo/GAZ_00027223 -->

    <owl:NamedIndividual rdf:about="http://purl.obolibrary.org/obo/GAZ_00027223">
        <obo:RO_0001025 rdf:resource="http://purl.obolibrary.org/obo/GAZ_00014885"/>
        <obo:IAO_0000115>A sum of Khovsgol aimag.</obo:IAO_0000115>
        <oboInOwl:hasOBONamespace>GAZ</oboInOwl:hasOBONamespace>
        <oboInOwl:id>GAZ:00027223</oboInOwl:id>
        <rdfs:label>Bayanzurkh District</rdfs:label>
    </owl:NamedIndividual>
    


    <!-- http://purl.obolibrary.org/obo/GAZ_00027224 -->

    <owl:NamedIndividual rdf:about="http://purl.obolibrary.org/obo/GAZ_00027224">
        <obo:RO_0001025 rdf:resource="http://purl.obolibrary.org/obo/GAZ_00014885"/>
        <obo:IAO_0000115>A sum of Khovsgol aimag. The Galt sum was founded, under the name Ider and as part of Arkhangai aimag, in 1931. It became part of Khovsgol aimag, in 1956 it was joined to Chandmani sum, in 1959 it was reestablished under the name Galt. In 1963, the Zurkh sum became part of Galt.</obo:IAO_0000115>
        <oboInOwl:hasOBONamespace>GAZ</oboInOwl:hasOBONamespace>
        <oboInOwl:id>GAZ:00027224</oboInOwl:id>
        <rdfs:label>Galt District</rdfs:label>
    </owl:NamedIndividual>
    


    <!-- http://purl.obolibrary.org/obo/GAZ_00027225 -->

    <owl:NamedIndividual rdf:about="http://purl.obolibrary.org/obo/GAZ_00027225">
        <obo:RO_0001025 rdf:resource="http://purl.obolibrary.org/obo/GAZ_00014885"/>
        <obo:IAO_0000115>A sum of Khovsgol aimag.</obo:IAO_0000115>
        <oboInOwl:hasOBONamespace>GAZ</oboInOwl:hasOBONamespace>
        <oboInOwl:id>GAZ:00027225</oboInOwl:id>
        <rdfs:label>Tosontsengel District</rdfs:label>
    </owl:NamedIndividual>
    


    <!-- http://purl.obolibrary.org/obo/GAZ_00027226 -->

    <owl:NamedIndividual rdf:about="http://purl.obolibrary.org/obo/GAZ_00027226">
        <obo:RO_0001025 rdf:resource="http://purl.obolibrary.org/obo/GAZ_00014885"/>
        <obo:IAO_0000115>A sum of Khovsgol aimag.</obo:IAO_0000115>
        <oboInOwl:hasOBONamespace>GAZ</oboInOwl:hasOBONamespace>
        <oboInOwl:id>GAZ:00027226</oboInOwl:id>
        <rdfs:label>Tomorbulag District</rdfs:label>
    </owl:NamedIndividual>
    


    <!-- http://purl.obolibrary.org/obo/GAZ_00027227 -->

    <owl:NamedIndividual rdf:about="http://purl.obolibrary.org/obo/GAZ_00027227">
        <obo:RO_0001025 rdf:resource="http://purl.obolibrary.org/obo/GAZ_00014885"/>
        <obo:IAO_0000115>A sum of Khovsgol aimag.</obo:IAO_0000115>
        <oboInOwl:hasOBONamespace>GAZ</oboInOwl:hasOBONamespace>
        <oboInOwl:id>GAZ:00027227</oboInOwl:id>
        <rdfs:label>Tsagaan-Uul District</rdfs:label>
    </owl:NamedIndividual>
    


    <!-- http://purl.obolibrary.org/obo/GAZ_00027228 -->

    <owl:NamedIndividual rdf:about="http://purl.obolibrary.org/obo/GAZ_00027228">
        <obo:RO_0001025 rdf:resource="http://purl.obolibrary.org/obo/GAZ_00014885"/>
        <obo:IAO_0000115>The administrative center of Khovsgol Aimag (province) in northern Mongolia.</obo:IAO_0000115>
        <oboInOwl:hasOBONamespace>GAZ</oboInOwl:hasOBONamespace>
        <oboInOwl:id>GAZ:00027228</oboInOwl:id>
        <rdfs:label>Moron City</rdfs:label>
    </owl:NamedIndividual>
    


    <!-- http://purl.obolibrary.org/obo/GAZ_00027229 -->

    <owl:NamedIndividual rdf:about="http://purl.obolibrary.org/obo/GAZ_00027229">
        <obo:RO_0001025 rdf:resource="http://purl.obolibrary.org/obo/GAZ_00014885"/>
        <obo:IAO_0000115>A sum of Khovsgol aimag. The Chandmani-Ondor sum was founded, together with the whole Khovsgol aimag. In 1956 it was joined with Tsagaan-Uur, but became separate again in 1959.</obo:IAO_0000115>
        <oboInOwl:hasOBONamespace>GAZ</oboInOwl:hasOBONamespace>
        <oboInOwl:id>GAZ:00027229</oboInOwl:id>
        <rdfs:label>Chandmani-Ondor District</rdfs:label>
    </owl:NamedIndividual>
    


    <!-- http://purl.obolibrary.org/obo/GAZ_00027230 -->

    <owl:NamedIndividual rdf:about="http://purl.obolibrary.org/obo/GAZ_00027230">
        <obo:RO_0001025 rdf:resource="http://purl.obolibrary.org/obo/GAZ_00014885"/>
        <obo:IAO_0000115>A sum of Khovsgol aimag.</obo:IAO_0000115>
        <oboInOwl:hasOBONamespace>GAZ</oboInOwl:hasOBONamespace>
        <oboInOwl:id>GAZ:00027230</oboInOwl:id>
        <rdfs:label>Tarialan District</rdfs:label>
    </owl:NamedIndividual>
    


    <!-- http://purl.obolibrary.org/obo/GAZ_00027231 -->

    <owl:NamedIndividual rdf:about="http://purl.obolibrary.org/obo/GAZ_00027231">
        <rdf:type rdf:resource="http://purl.obolibrary.org/obo/ENVO_00000004"/>
        <obo:RO_0001025 rdf:resource="http://purl.obolibrary.org/obo/GAZ_00014883"/>
        <obo:IAO_0000115>A sum (district) of Khovd Province in western Mongolia.</obo:IAO_0000115>
        <oboInOwl:hasOBONamespace>GAZ</oboInOwl:hasOBONamespace>
        <oboInOwl:id>GAZ:00027231</oboInOwl:id>
        <rdfs:label>Zereg District</rdfs:label>
    </owl:NamedIndividual>
    


    <!-- http://purl.obolibrary.org/obo/GAZ_00027232 -->

    <owl:NamedIndividual rdf:about="http://purl.obolibrary.org/obo/GAZ_00027232">
        <obo:RO_0001025 rdf:resource="http://purl.obolibrary.org/obo/GAZ_00014885"/>
        <obo:IAO_0000115>A sum of Khovsgol Aimag. The Erdenebulgan sum was founded, together with the whole Khovsgol Aimag, in 1931. In 1956, it was joined with Tsagaan-Uur. In 1959, the Eg-Uur farm was founded, and Erdenebulgan became separate again. In 1975, the sum was dissolved once more, the state farm became part of another farm, but both the sum and the farm were reestablished again in 1985.</obo:IAO_0000115>
        <oboInOwl:hasOBONamespace>GAZ</oboInOwl:hasOBONamespace>
        <oboInOwl:id>GAZ:00027232</oboInOwl:id>
        <rdfs:label>Erdenebulgan District</rdfs:label>
    </owl:NamedIndividual>
    


    <!-- http://purl.obolibrary.org/obo/GAZ_00027233 -->

    <owl:NamedIndividual rdf:about="http://purl.obolibrary.org/obo/GAZ_00027233">
        <rdf:type rdf:resource="http://purl.obolibrary.org/obo/ENVO_00000004"/>
        <obo:RO_0001025 rdf:resource="http://purl.obolibrary.org/obo/GAZ_00014883"/>
        <obo:IAO_0000115>A sum (district) of Khovd Province in western Mongolia.</obo:IAO_0000115>
        <oboInOwl:hasOBONamespace>GAZ</oboInOwl:hasOBONamespace>
        <oboInOwl:id>GAZ:00027233</oboInOwl:id>
        <rdfs:label>Tsetseg District</rdfs:label>
    </owl:NamedIndividual>
    


    <!-- http://purl.obolibrary.org/obo/GAZ_00027234 -->

    <owl:NamedIndividual rdf:about="http://purl.obolibrary.org/obo/GAZ_00027234">
        <obo:RO_0001025 rdf:resource="http://purl.obolibrary.org/obo/GAZ_00014885"/>
        <obo:IAO_0000115>A sum of Khovsgol aimag. The Tsagaannuur sum was split off from Renchinlkhumbe, Khovsgol in 1985.</obo:IAO_0000115>
        <oboInOwl:hasOBONamespace>GAZ</oboInOwl:hasOBONamespace>
        <oboInOwl:id>GAZ:00027234</oboInOwl:id>
        <rdfs:label>Tsagaannuur District</rdfs:label>
    </owl:NamedIndividual>
    


    <!-- http://purl.obolibrary.org/obo/GAZ_00027235 -->

    <owl:NamedIndividual rdf:about="http://purl.obolibrary.org/obo/GAZ_00027235">
        <obo:RO_0001025 rdf:resource="http://purl.obolibrary.org/obo/GAZ_00014885"/>
        <obo:IAO_0000115>A sum of Khovsgol aimag. The Shine-Ider sum was founded in 1923 as Chandmana sum of the Tsetserleg Mandal Uulyn aimag&apos;s Chandmana-Olziit Dalain khoshuu. In 1931, it became the Chandmana sum of the newly founded Arkhangai aimag. In 1942 it became part of Khovsgol aimag, and was renamed Shine-Ider in 1956.</obo:IAO_0000115>
        <oboInOwl:hasOBONamespace>GAZ</oboInOwl:hasOBONamespace>
        <oboInOwl:id>GAZ:00027235</oboInOwl:id>
        <rdfs:label>Shine-Ider District</rdfs:label>
    </owl:NamedIndividual>
    


    <!-- http://purl.obolibrary.org/obo/GAZ_00027236 -->

    <owl:NamedIndividual rdf:about="http://purl.obolibrary.org/obo/GAZ_00027236">
        <obo:RO_0001025 rdf:resource="http://purl.obolibrary.org/obo/GAZ_00014885"/>
        <obo:IAO_0000115>A sum of Khovsgol aimag.</obo:IAO_0000115>
        <oboInOwl:hasOBONamespace>GAZ</oboInOwl:hasOBONamespace>
        <oboInOwl:id>GAZ:00027236</oboInOwl:id>
        <rdfs:label>Jargalant District</rdfs:label>
    </owl:NamedIndividual>
    


    <!-- http://purl.obolibrary.org/obo/GAZ_00027237 -->

    <owl:NamedIndividual rdf:about="http://purl.obolibrary.org/obo/GAZ_00027237">
        <rdf:type rdf:resource="http://purl.obolibrary.org/obo/ENVO_00000004"/>
        <obo:RO_0001025 rdf:resource="http://purl.obolibrary.org/obo/GAZ_00014883"/>
        <obo:IAO_0000115>A sum (district) of Khovd Province in western Mongolia.</obo:IAO_0000115>
        <oboInOwl:hasOBONamespace>GAZ</oboInOwl:hasOBONamespace>
        <oboInOwl:id>GAZ:00027237</oboInOwl:id>
        <rdfs:label>Uyench District</rdfs:label>
    </owl:NamedIndividual>
    


    <!-- http://purl.obolibrary.org/obo/GAZ_00027238 -->

    <owl:NamedIndividual rdf:about="http://purl.obolibrary.org/obo/GAZ_00027238">
        <rdf:type rdf:resource="http://purl.obolibrary.org/obo/ENVO_00000004"/>
        <obo:RO_0001025 rdf:resource="http://purl.obolibrary.org/obo/GAZ_00014883"/>
        <obo:IAO_0000115>A sum (district) of Khovd Province in western Mongolia.</obo:IAO_0000115>
        <oboInOwl:hasOBONamespace>GAZ</oboInOwl:hasOBONamespace>
        <oboInOwl:id>GAZ:00027238</oboInOwl:id>
        <rdfs:label>Erdeneburen District</rdfs:label>
    </owl:NamedIndividual>
    


    <!-- http://purl.obolibrary.org/obo/GAZ_00027239 -->

    <owl:NamedIndividual rdf:about="http://purl.obolibrary.org/obo/GAZ_00027239">
        <rdf:type rdf:resource="http://purl.obolibrary.org/obo/ENVO_00000004"/>
        <obo:RO_0001025 rdf:resource="http://purl.obolibrary.org/obo/GAZ_00014883"/>
        <obo:IAO_0000115>A sum (district) of Khovd Province in western Mongolia.</obo:IAO_0000115>
        <oboInOwl:hasOBONamespace>GAZ</oboInOwl:hasOBONamespace>
        <oboInOwl:id>GAZ:00027239</oboInOwl:id>
        <rdfs:label>Darvi District</rdfs:label>
    </owl:NamedIndividual>
    


    <!-- http://purl.obolibrary.org/obo/GAZ_00027240 -->

    <owl:NamedIndividual rdf:about="http://purl.obolibrary.org/obo/GAZ_00027240">
        <rdf:type rdf:resource="http://purl.obolibrary.org/obo/ENVO_00000004"/>
        <obo:RO_0001025 rdf:resource="http://purl.obolibrary.org/obo/GAZ_00014883"/>
        <obo:IAO_0000115>A sum (district) of Khovd Province in western Mongolia.</obo:IAO_0000115>
        <oboInOwl:hasOBONamespace>GAZ</oboInOwl:hasOBONamespace>
        <oboInOwl:id>GAZ:00027240</oboInOwl:id>
        <rdfs:label>Bulgan District</rdfs:label>
    </owl:NamedIndividual>
    


    <!-- http://purl.obolibrary.org/obo/GAZ_00027241 -->

    <owl:NamedIndividual rdf:about="http://purl.obolibrary.org/obo/GAZ_00027241">
        <rdf:type rdf:resource="http://purl.obolibrary.org/obo/ENVO_00000004"/>
        <obo:RO_0001025 rdf:resource="http://purl.obolibrary.org/obo/GAZ_00014883"/>
        <obo:IAO_0000115>A sum (district) of Khovd Province in western Mongolia.</obo:IAO_0000115>
        <oboInOwl:hasOBONamespace>GAZ</oboInOwl:hasOBONamespace>
        <oboInOwl:id>GAZ:00027241</oboInOwl:id>
        <rdfs:label>Mankhan District</rdfs:label>
    </owl:NamedIndividual>
    


    <!-- http://purl.obolibrary.org/obo/GAZ_00027242 -->

    <owl:NamedIndividual rdf:about="http://purl.obolibrary.org/obo/GAZ_00027242">
        <obo:RO_0001025 rdf:resource="http://purl.obolibrary.org/obo/GAZ_00014885"/>
        <obo:IAO_0000115>A sum of Khovsgol aimag.</obo:IAO_0000115>
        <oboInOwl:hasOBONamespace>GAZ</oboInOwl:hasOBONamespace>
        <oboInOwl:id>GAZ:00027242</oboInOwl:id>
        <rdfs:label>Tsagaan-Uur District</rdfs:label>
    </owl:NamedIndividual>
    


    <!-- http://purl.obolibrary.org/obo/GAZ_00027243 -->

    <owl:NamedIndividual rdf:about="http://purl.obolibrary.org/obo/GAZ_00027243">
        <obo:RO_0001025 rdf:resource="http://purl.obolibrary.org/obo/GAZ_00014885"/>
        <obo:IAO_0000115>A sum of Khovsgol aimag.</obo:IAO_0000115>
        <oboInOwl:hasOBONamespace>GAZ</oboInOwl:hasOBONamespace>
        <oboInOwl:id>GAZ:00027243</oboInOwl:id>
        <rdfs:label>Ikh-Uul District</rdfs:label>
    </owl:NamedIndividual>
    


    <!-- http://purl.obolibrary.org/obo/GAZ_00027244 -->

    <owl:NamedIndividual rdf:about="http://purl.obolibrary.org/obo/GAZ_00027244">
        <rdf:type rdf:resource="http://purl.obolibrary.org/obo/ENVO_00000004"/>
        <obo:RO_0001025 rdf:resource="http://purl.obolibrary.org/obo/GAZ_00014883"/>
        <obo:IAO_0000115>A sum (district) of Khovd Province in western Mongolia.</obo:IAO_0000115>
        <oboInOwl:hasOBONamespace>GAZ</oboInOwl:hasOBONamespace>
        <oboInOwl:id>GAZ:00027244</oboInOwl:id>
        <rdfs:label>Drgon District</rdfs:label>
    </owl:NamedIndividual>
    


    <!-- http://purl.obolibrary.org/obo/GAZ_00027245 -->

    <owl:NamedIndividual rdf:about="http://purl.obolibrary.org/obo/GAZ_00027245">
        <rdf:type rdf:resource="http://purl.obolibrary.org/obo/ENVO_00000004"/>
        <obo:RO_0001025 rdf:resource="http://purl.obolibrary.org/obo/GAZ_00014883"/>
        <obo:IAO_0000115>A sum (district) of Khovd Province in western Mongolia.</obo:IAO_0000115>
        <oboInOwl:hasOBONamespace>GAZ</oboInOwl:hasOBONamespace>
        <oboInOwl:id>GAZ:00027245</oboInOwl:id>
        <rdfs:label>Jargalant District</rdfs:label>
    </owl:NamedIndividual>
    


    <!-- http://purl.obolibrary.org/obo/GAZ_00027246 -->

    <owl:NamedIndividual rdf:about="http://purl.obolibrary.org/obo/GAZ_00027246">
        <rdf:type rdf:resource="http://purl.obolibrary.org/obo/ENVO_00000004"/>
        <obo:RO_0001025 rdf:resource="http://purl.obolibrary.org/obo/GAZ_00014883"/>
        <obo:IAO_0000115>A sum (district) of Khovd Province in western Mongolia.</obo:IAO_0000115>
        <oboInOwl:hasOBONamespace>GAZ</oboInOwl:hasOBONamespace>
        <oboInOwl:id>GAZ:00027246</oboInOwl:id>
        <rdfs:label>Buyant District</rdfs:label>
    </owl:NamedIndividual>
    


    <!-- http://purl.obolibrary.org/obo/GAZ_00027247 -->

    <owl:NamedIndividual rdf:about="http://purl.obolibrary.org/obo/GAZ_00027247">
        <obo:RO_0001025 rdf:resource="http://purl.obolibrary.org/obo/GAZ_00014885"/>
        <obo:IAO_0000115>A sum of Khovsgol aimag.</obo:IAO_0000115>
        <oboInOwl:hasOBONamespace>GAZ</oboInOwl:hasOBONamespace>
        <oboInOwl:id>GAZ:00027247</oboInOwl:id>
        <rdfs:label>Burentogtokh District</rdfs:label>
    </owl:NamedIndividual>
    


    <!-- http://purl.obolibrary.org/obo/GAZ_00027248 -->

    <owl:NamedIndividual rdf:about="http://purl.obolibrary.org/obo/GAZ_00027248">
        <obo:RO_0001025 rdf:resource="http://purl.obolibrary.org/obo/GAZ_00014885"/>
        <obo:IAO_0000115>A sum of Khovsgol aimag.</obo:IAO_0000115>
        <oboInOwl:hasOBONamespace>GAZ</oboInOwl:hasOBONamespace>
        <oboInOwl:id>GAZ:00027248</oboInOwl:id>
        <rdfs:label>Tsetserleg District</rdfs:label>
    </owl:NamedIndividual>
    


    <!-- http://purl.obolibrary.org/obo/GAZ_00027249 -->

    <owl:NamedIndividual rdf:about="http://purl.obolibrary.org/obo/GAZ_00027249">
        <obo:RO_0001025 rdf:resource="http://purl.obolibrary.org/obo/GAZ_00014885"/>
        <obo:IAO_0000115>A sum of Khovsgol aimag. Lake Khovsgol borders the sum to the north.</obo:IAO_0000115>
        <oboInOwl:hasOBONamespace>GAZ</oboInOwl:hasOBONamespace>
        <oboInOwl:id>GAZ:00027249</oboInOwl:id>
        <rdfs:label>Alag-Erdene District</rdfs:label>
    </owl:NamedIndividual>
    


    <!-- http://purl.obolibrary.org/obo/GAZ_00027250 -->

    <owl:NamedIndividual rdf:about="http://purl.obolibrary.org/obo/GAZ_00027250">
        <rdf:type rdf:resource="http://purl.obolibrary.org/obo/ENVO_00000004"/>
        <obo:RO_0001025 rdf:resource="http://purl.obolibrary.org/obo/GAZ_00014883"/>
        <obo:IAO_0000115>A sum (district) of Khovd Province in western Mongolia.</obo:IAO_0000115>
        <oboInOwl:hasOBONamespace>GAZ</oboInOwl:hasOBONamespace>
        <oboInOwl:id>GAZ:00027250</oboInOwl:id>
        <rdfs:label>Monkhkhairkhan District</rdfs:label>
    </owl:NamedIndividual>
    


    <!-- http://purl.obolibrary.org/obo/GAZ_00027251 -->

    <owl:NamedIndividual rdf:about="http://purl.obolibrary.org/obo/GAZ_00027251">
        <rdf:type rdf:resource="http://purl.obolibrary.org/obo/ENVO_00000004"/>
        <obo:RO_0001025 rdf:resource="http://purl.obolibrary.org/obo/GAZ_00014883"/>
        <obo:IAO_0000115>A sum (district) of Khovd Province in western Mongolia.</obo:IAO_0000115>
        <oboInOwl:hasOBONamespace>GAZ</oboInOwl:hasOBONamespace>
        <oboInOwl:id>GAZ:00027251</oboInOwl:id>
        <rdfs:label>Duut District</rdfs:label>
    </owl:NamedIndividual>
    


    <!-- http://purl.obolibrary.org/obo/GAZ_00027252 -->

    <owl:NamedIndividual rdf:about="http://purl.obolibrary.org/obo/GAZ_00027252">
        <rdf:type rdf:resource="http://purl.obolibrary.org/obo/ENVO_00000004"/>
        <obo:RO_0001025 rdf:resource="http://purl.obolibrary.org/obo/GAZ_00014883"/>
        <obo:IAO_0000115>A sum (district) of Khovd Province in western Mongolia.</obo:IAO_0000115>
        <oboInOwl:hasOBONamespace>GAZ</oboInOwl:hasOBONamespace>
        <oboInOwl:id>GAZ:00027252</oboInOwl:id>
        <rdfs:label>Chandmani District</rdfs:label>
    </owl:NamedIndividual>
    


    <!-- http://purl.obolibrary.org/obo/GAZ_00027253 -->

    <owl:NamedIndividual rdf:about="http://purl.obolibrary.org/obo/GAZ_00027253">
        <rdf:type rdf:resource="http://purl.obolibrary.org/obo/ENVO_00000004"/>
        <obo:RO_0001025 rdf:resource="http://purl.obolibrary.org/obo/GAZ_00014883"/>
        <obo:IAO_0000115>A sum (district) of Khovd Province in western Mongolia.</obo:IAO_0000115>
        <oboInOwl:hasOBONamespace>GAZ</oboInOwl:hasOBONamespace>
        <oboInOwl:id>GAZ:00027253</oboInOwl:id>
        <rdfs:label>Most District</rdfs:label>
    </owl:NamedIndividual>
    


    <!-- http://purl.obolibrary.org/obo/GAZ_00027254 -->

    <owl:NamedIndividual rdf:about="http://purl.obolibrary.org/obo/GAZ_00027254">
        <rdf:type rdf:resource="http://purl.obolibrary.org/obo/ENVO_00000004"/>
        <obo:RO_0001025 rdf:resource="http://purl.obolibrary.org/obo/GAZ_00014883"/>
        <obo:IAO_0000115>A sum (district) of Khovd Province in western Mongolia.</obo:IAO_0000115>
        <oboInOwl:hasOBONamespace>GAZ</oboInOwl:hasOBONamespace>
        <oboInOwl:id>GAZ:00027254</oboInOwl:id>
        <rdfs:label>Khovd District</rdfs:label>
    </owl:NamedIndividual>
    


    <!-- http://purl.obolibrary.org/obo/GAZ_00027255 -->

    <owl:NamedIndividual rdf:about="http://purl.obolibrary.org/obo/GAZ_00027255">
        <obo:RO_0001025 rdf:resource="http://purl.obolibrary.org/obo/GAZ_00014885"/>
        <obo:IAO_0000115>A sum of Khovsgol aimag.</obo:IAO_0000115>
        <oboInOwl:hasOBONamespace>GAZ</oboInOwl:hasOBONamespace>
        <oboInOwl:id>GAZ:00027255</oboInOwl:id>
        <rdfs:label>Arbulag District</rdfs:label>
    </owl:NamedIndividual>
    


    <!-- http://purl.obolibrary.org/obo/GAZ_00027256 -->

    <owl:NamedIndividual rdf:about="http://purl.obolibrary.org/obo/GAZ_00027256">
        <obo:RO_0001025 rdf:resource="http://purl.obolibrary.org/obo/GAZ_00014885"/>
        <obo:IAO_0000115>A sum of Khovsgol aimag.</obo:IAO_0000115>
        <oboInOwl:hasOBONamespace>GAZ</oboInOwl:hasOBONamespace>
        <oboInOwl:id>GAZ:00027256</oboInOwl:id>
        <rdfs:label>Renchinlkhumbe District</rdfs:label>
    </owl:NamedIndividual>
    


    <!-- http://purl.obolibrary.org/obo/GAZ_00027257 -->

    <owl:NamedIndividual rdf:about="http://purl.obolibrary.org/obo/GAZ_00027257">
        <rdf:type rdf:resource="http://purl.obolibrary.org/obo/ENVO_00000004"/>
        <obo:RO_0001025 rdf:resource="http://purl.obolibrary.org/obo/GAZ_00014883"/>
        <obo:IAO_0000115>A sum (district) of Khovd Province in western Mongolia.</obo:IAO_0000115>
        <oboInOwl:hasOBONamespace>GAZ</oboInOwl:hasOBONamespace>
        <oboInOwl:id>GAZ:00027257</oboInOwl:id>
        <rdfs:label>Myangad District</rdfs:label>
    </owl:NamedIndividual>
    


    <!-- http://purl.obolibrary.org/obo/GAZ_00027258 -->

    <owl:NamedIndividual rdf:about="http://purl.obolibrary.org/obo/GAZ_00027258">
        <obo:RO_0001025 rdf:resource="http://purl.obolibrary.org/obo/GAZ_00014885"/>
        <obo:IAO_0000115>A sum of Khovsgol aimag. The Tunel sum was founded in 1952 from parts of the Buren, Tosontsengel, Erdenebulgan, and Alag-Erdene sums. In 1956, it became part of Burentogtokh sum, but was separated again in 1959.</obo:IAO_0000115>
        <oboInOwl:hasOBONamespace>GAZ</oboInOwl:hasOBONamespace>
        <oboInOwl:id>GAZ:00027258</oboInOwl:id>
        <rdfs:label>Tunel District</rdfs:label>
    </owl:NamedIndividual>
    


    <!-- http://purl.obolibrary.org/obo/GAZ_00027259 -->

    <owl:NamedIndividual rdf:about="http://purl.obolibrary.org/obo/GAZ_00027259">
        <obo:RO_0001025 rdf:resource="http://purl.obolibrary.org/obo/GAZ_00014885"/>
        <obo:IAO_0000115>A sum of Khovsgol aimag.</obo:IAO_0000115>
        <oboInOwl:hasOBONamespace>GAZ</oboInOwl:hasOBONamespace>
        <oboInOwl:id>GAZ:00027259</oboInOwl:id>
        <rdfs:label>Ulaan-Uul District</rdfs:label>
    </owl:NamedIndividual>
    


    <!-- http://purl.obolibrary.org/obo/GAZ_00027260 -->

    <owl:NamedIndividual rdf:about="http://purl.obolibrary.org/obo/GAZ_00027260">
        <obo:RO_0001025 rdf:resource="http://purl.obolibrary.org/obo/GAZ_00014886"/>
        <obo:IAO_0000115>The capital of Ovorkhangai Aimag (province) and one of the most central points of Mongolia.</obo:IAO_0000115>
        <oboInOwl:hasOBONamespace>GAZ</oboInOwl:hasOBONamespace>
        <oboInOwl:id>GAZ:00027260</oboInOwl:id>
        <rdfs:label>Arvaikheer District</rdfs:label>
    </owl:NamedIndividual>
    


    <!-- http://purl.obolibrary.org/obo/GAZ_00027261 -->

    <owl:NamedIndividual rdf:about="http://purl.obolibrary.org/obo/GAZ_00027261">
        <rdf:type rdf:resource="http://purl.obolibrary.org/obo/ENVO_00000004"/>
        <obo:RO_0001025 rdf:resource="http://purl.obolibrary.org/obo/GAZ_00014886"/>
        <obo:IAO_0000115>A sum (district) of Ovorkhangai Province in southern Mongolia.</obo:IAO_0000115>
        <oboInOwl:hasOBONamespace>GAZ</oboInOwl:hasOBONamespace>
        <oboInOwl:id>GAZ:00027261</oboInOwl:id>
        <rdfs:label>Guchin-Us District</rdfs:label>
    </owl:NamedIndividual>
    


    <!-- http://purl.obolibrary.org/obo/GAZ_00027262 -->

    <owl:NamedIndividual rdf:about="http://purl.obolibrary.org/obo/GAZ_00027262">
        <rdf:type rdf:resource="http://purl.obolibrary.org/obo/ENVO_00000004"/>
        <obo:RO_0001025 rdf:resource="http://purl.obolibrary.org/obo/GAZ_00014882"/>
        <obo:IAO_0000115>A sum (district) of Omnogovi Province in southern Mongolia.</obo:IAO_0000115>
        <oboInOwl:hasOBONamespace>GAZ</oboInOwl:hasOBONamespace>
        <oboInOwl:id>GAZ:00027262</oboInOwl:id>
        <rdfs:label>Bayan-Ovoo District</rdfs:label>
    </owl:NamedIndividual>
    


    <!-- http://purl.obolibrary.org/obo/GAZ_00027263 -->

    <owl:NamedIndividual rdf:about="http://purl.obolibrary.org/obo/GAZ_00027263">
        <rdf:type rdf:resource="http://purl.obolibrary.org/obo/ENVO_00000004"/>
        <obo:RO_0001025 rdf:resource="http://purl.obolibrary.org/obo/GAZ_00014882"/>
        <obo:IAO_0000115>A sum (district) of Omnogovi Province in southern Mongolia.</obo:IAO_0000115>
        <oboInOwl:hasOBONamespace>GAZ</oboInOwl:hasOBONamespace>
        <oboInOwl:id>GAZ:00027263</oboInOwl:id>
        <rdfs:label>Sevrei District</rdfs:label>
    </owl:NamedIndividual>
    


    <!-- http://purl.obolibrary.org/obo/GAZ_00027264 -->

    <owl:NamedIndividual rdf:about="http://purl.obolibrary.org/obo/GAZ_00027264">
        <rdf:type rdf:resource="http://purl.obolibrary.org/obo/ENVO_00000004"/>
        <obo:RO_0001025 rdf:resource="http://purl.obolibrary.org/obo/GAZ_00014886"/>
        <obo:IAO_0000115>A sum (district) of Ovorkhangai Province in southern Mongolia.</obo:IAO_0000115>
        <oboInOwl:hasOBONamespace>GAZ</oboInOwl:hasOBONamespace>
        <oboInOwl:id>GAZ:00027264</oboInOwl:id>
        <rdfs:label>Bat-Olzii District</rdfs:label>
    </owl:NamedIndividual>
    


    <!-- http://purl.obolibrary.org/obo/GAZ_00027265 -->

    <owl:NamedIndividual rdf:about="http://purl.obolibrary.org/obo/GAZ_00027265">
        <rdf:type rdf:resource="http://purl.obolibrary.org/obo/ENVO_00000004"/>
        <obo:RO_0001025 rdf:resource="http://purl.obolibrary.org/obo/GAZ_00014884"/>
        <obo:IAO_0000115>A sum (district) of Orkhon Province in northern Mongolia.</obo:IAO_0000115>
        <oboInOwl:hasOBONamespace>GAZ</oboInOwl:hasOBONamespace>
        <oboInOwl:id>GAZ:00027265</oboInOwl:id>
        <rdfs:label>Bayan-Ondor District</rdfs:label>
    </owl:NamedIndividual>
    


    <!-- http://purl.obolibrary.org/obo/GAZ_00027266 -->

    <owl:NamedIndividual rdf:about="http://purl.obolibrary.org/obo/GAZ_00027266">
        <rdf:type rdf:resource="http://purl.obolibrary.org/obo/ENVO_00000004"/>
        <obo:RO_0001025 rdf:resource="http://purl.obolibrary.org/obo/GAZ_00014886"/>
        <obo:IAO_0000115>A sum (district) of Ovorkhangai Province in southern Mongolia.</obo:IAO_0000115>
        <oboInOwl:hasOBONamespace>GAZ</oboInOwl:hasOBONamespace>
        <oboInOwl:id>GAZ:00027266</oboInOwl:id>
        <rdfs:label>Olziit District</rdfs:label>
    </owl:NamedIndividual>
    


    <!-- http://purl.obolibrary.org/obo/GAZ_00027267 -->

    <owl:NamedIndividual rdf:about="http://purl.obolibrary.org/obo/GAZ_00027267">
        <rdf:type rdf:resource="http://purl.obolibrary.org/obo/ENVO_00000004"/>
        <obo:RO_0001025 rdf:resource="http://purl.obolibrary.org/obo/GAZ_00014886"/>
        <obo:IAO_0000115>A sum (district) of Ovorkhangai Province in southern Mongolia.</obo:IAO_0000115>
        <oboInOwl:hasOBONamespace>GAZ</oboInOwl:hasOBONamespace>
        <oboInOwl:id>GAZ:00027267</oboInOwl:id>
        <rdfs:label>Khujirt District</rdfs:label>
    </owl:NamedIndividual>
    


    <!-- http://purl.obolibrary.org/obo/GAZ_00027268 -->

    <owl:NamedIndividual rdf:about="http://purl.obolibrary.org/obo/GAZ_00027268">
        <rdf:type rdf:resource="http://purl.obolibrary.org/obo/ENVO_00000004"/>
        <obo:RO_0001025 rdf:resource="http://purl.obolibrary.org/obo/GAZ_00014882"/>
        <obo:IAO_0000115>A sum (district) of Omnogovi Province in southern Mongolia.</obo:IAO_0000115>
        <oboInOwl:hasOBONamespace>GAZ</oboInOwl:hasOBONamespace>
        <oboInOwl:id>GAZ:00027268</oboInOwl:id>
        <rdfs:label>Noyon District</rdfs:label>
    </owl:NamedIndividual>
    


    <!-- http://purl.obolibrary.org/obo/GAZ_00027269 -->

    <owl:NamedIndividual rdf:about="http://purl.obolibrary.org/obo/GAZ_00027269">
        <rdf:type rdf:resource="http://purl.obolibrary.org/obo/ENVO_00000004"/>
        <obo:RO_0001025 rdf:resource="http://purl.obolibrary.org/obo/GAZ_00014886"/>
        <obo:IAO_0000115>A sum (district) of Ovorkhangai Province in southern Mongolia.</obo:IAO_0000115>
        <oboInOwl:hasOBONamespace>GAZ</oboInOwl:hasOBONamespace>
        <oboInOwl:id>GAZ:00027269</oboInOwl:id>
        <rdfs:label>Taragt District</rdfs:label>
    </owl:NamedIndividual>
    


    <!-- http://purl.obolibrary.org/obo/GAZ_00027270 -->

    <owl:NamedIndividual rdf:about="http://purl.obolibrary.org/obo/GAZ_00027270">
        <rdf:type rdf:resource="http://purl.obolibrary.org/obo/ENVO_00000004"/>
        <obo:RO_0001025 rdf:resource="http://purl.obolibrary.org/obo/GAZ_00014886"/>
        <obo:IAO_0000115>A sum (district) of Ovorkhangai Province in southern Mongolia.</obo:IAO_0000115>
        <oboInOwl:hasOBONamespace>GAZ</oboInOwl:hasOBONamespace>
        <oboInOwl:id>GAZ:00027270</oboInOwl:id>
        <rdfs:label>Togrog District</rdfs:label>
    </owl:NamedIndividual>
    


    <!-- http://purl.obolibrary.org/obo/GAZ_00027271 -->

    <owl:NamedIndividual rdf:about="http://purl.obolibrary.org/obo/GAZ_00027271">
        <rdf:type rdf:resource="http://purl.obolibrary.org/obo/ENVO_00000004"/>
        <obo:RO_0001025 rdf:resource="http://purl.obolibrary.org/obo/GAZ_00014882"/>
        <obo:IAO_0000115>A sum (district) of Omnogovi Province in southern Mongolia.</obo:IAO_0000115>
        <oboInOwl:hasOBONamespace>GAZ</oboInOwl:hasOBONamespace>
        <oboInOwl:id>GAZ:00027271</oboInOwl:id>
        <rdfs:label>Khurmen District</rdfs:label>
    </owl:NamedIndividual>
    


    <!-- http://purl.obolibrary.org/obo/GAZ_00027272 -->

    <owl:NamedIndividual rdf:about="http://purl.obolibrary.org/obo/GAZ_00027272">
        <rdf:type rdf:resource="http://purl.obolibrary.org/obo/ENVO_00000004"/>
        <obo:RO_0001025 rdf:resource="http://purl.obolibrary.org/obo/GAZ_00014882"/>
        <obo:IAO_0000115>A sum (district) of Omnogovi Province in southern Mongolia.</obo:IAO_0000115>
        <oboInOwl:hasOBONamespace>GAZ</oboInOwl:hasOBONamespace>
        <oboInOwl:id>GAZ:00027272</oboInOwl:id>
        <rdfs:label>Bulgan District</rdfs:label>
    </owl:NamedIndividual>
    


    <!-- http://purl.obolibrary.org/obo/GAZ_00027273 -->

    <owl:NamedIndividual rdf:about="http://purl.obolibrary.org/obo/GAZ_00027273">
        <rdf:type rdf:resource="http://purl.obolibrary.org/obo/ENVO_00000004"/>
        <obo:RO_0001025 rdf:resource="http://purl.obolibrary.org/obo/GAZ_00014882"/>
        <obo:IAO_0000115>A sum (district) of Omnogovi Province in southern Mongolia.</obo:IAO_0000115>
        <oboInOwl:hasOBONamespace>GAZ</oboInOwl:hasOBONamespace>
        <oboInOwl:id>GAZ:00027273</oboInOwl:id>
        <rdfs:label>Nomgon District</rdfs:label>
    </owl:NamedIndividual>
    


    <!-- http://purl.obolibrary.org/obo/GAZ_00027274 -->

    <owl:NamedIndividual rdf:about="http://purl.obolibrary.org/obo/GAZ_00027274">
        <rdf:type rdf:resource="http://purl.obolibrary.org/obo/ENVO_00000004"/>
        <obo:RO_0001025 rdf:resource="http://purl.obolibrary.org/obo/GAZ_00014882"/>
        <obo:IAO_0000115>A sum (district) of Omnogovi Province in southern Mongolia.</obo:IAO_0000115>
        <oboInOwl:hasOBONamespace>GAZ</oboInOwl:hasOBONamespace>
        <oboInOwl:id>GAZ:00027274</oboInOwl:id>
        <rdfs:label>Gurvan tes District</rdfs:label>
    </owl:NamedIndividual>
    


    <!-- http://purl.obolibrary.org/obo/GAZ_00027275 -->

    <owl:NamedIndividual rdf:about="http://purl.obolibrary.org/obo/GAZ_00027275">
        <rdf:type rdf:resource="http://purl.obolibrary.org/obo/ENVO_00000004"/>
        <obo:RO_0001025 rdf:resource="http://purl.obolibrary.org/obo/GAZ_00014882"/>
        <obo:IAO_0000115>A sum (district) of Omnogovi Province in southern Mongolia.</obo:IAO_0000115>
        <oboInOwl:hasOBONamespace>GAZ</oboInOwl:hasOBONamespace>
        <oboInOwl:id>GAZ:00027275</oboInOwl:id>
        <rdfs:label>Khanbogd District</rdfs:label>
    </owl:NamedIndividual>
    


    <!-- http://purl.obolibrary.org/obo/GAZ_00027276 -->

    <owl:NamedIndividual rdf:about="http://purl.obolibrary.org/obo/GAZ_00027276">
        <rdf:type rdf:resource="http://purl.obolibrary.org/obo/ENVO_00000004"/>
        <obo:RO_0001025 rdf:resource="http://purl.obolibrary.org/obo/GAZ_00014882"/>
        <obo:IAO_0000115>A sum (district) of Omnogovi Province in southern Mongolia.</obo:IAO_0000115>
        <oboInOwl:hasOBONamespace>GAZ</oboInOwl:hasOBONamespace>
        <oboInOwl:id>GAZ:00027276</oboInOwl:id>
        <rdfs:label>Bayandalai District</rdfs:label>
    </owl:NamedIndividual>
    


    <!-- http://purl.obolibrary.org/obo/GAZ_00027277 -->

    <owl:NamedIndividual rdf:about="http://purl.obolibrary.org/obo/GAZ_00027277">
        <rdf:type rdf:resource="http://purl.obolibrary.org/obo/ENVO_00000004"/>
        <obo:RO_0001025 rdf:resource="http://purl.obolibrary.org/obo/GAZ_00014886"/>
        <obo:IAO_0000115>A sum (district) of Ovorkhangai Province in southern Mongolia.</obo:IAO_0000115>
        <oboInOwl:hasOBONamespace>GAZ</oboInOwl:hasOBONamespace>
        <oboInOwl:id>GAZ:00027277</oboInOwl:id>
        <rdfs:label>Burd District</rdfs:label>
    </owl:NamedIndividual>
    


    <!-- http://purl.obolibrary.org/obo/GAZ_00027278 -->

    <owl:NamedIndividual rdf:about="http://purl.obolibrary.org/obo/GAZ_00027278">
        <rdf:type rdf:resource="http://purl.obolibrary.org/obo/ENVO_00000004"/>
        <obo:RO_0001025 rdf:resource="http://purl.obolibrary.org/obo/GAZ_00014882"/>
        <obo:IAO_0000115>A sum (district) of Omnogovi Province in southern Mongolia.</obo:IAO_0000115>
        <oboInOwl:hasOBONamespace>GAZ</oboInOwl:hasOBONamespace>
        <oboInOwl:id>GAZ:00027278</oboInOwl:id>
        <rdfs:label>Mandal-Ovoo District</rdfs:label>
    </owl:NamedIndividual>
    


    <!-- http://purl.obolibrary.org/obo/GAZ_00027279 -->

    <owl:NamedIndividual rdf:about="http://purl.obolibrary.org/obo/GAZ_00027279">
        <rdf:type rdf:resource="http://purl.obolibrary.org/obo/ENVO_00000004"/>
        <obo:RO_0001025 rdf:resource="http://purl.obolibrary.org/obo/GAZ_00014882"/>
        <obo:IAO_0000115>A sum (district) of Omnogovi Province in southern Mongolia.</obo:IAO_0000115>
        <oboInOwl:hasOBONamespace>GAZ</oboInOwl:hasOBONamespace>
        <oboInOwl:id>GAZ:00027279</oboInOwl:id>
        <rdfs:label>Khan khongor District</rdfs:label>
    </owl:NamedIndividual>
    


    <!-- http://purl.obolibrary.org/obo/GAZ_00027280 -->

    <owl:NamedIndividual rdf:about="http://purl.obolibrary.org/obo/GAZ_00027280">
        <rdf:type rdf:resource="http://purl.obolibrary.org/obo/ENVO_00000004"/>
        <obo:RO_0001025 rdf:resource="http://purl.obolibrary.org/obo/GAZ_00014882"/>
        <obo:IAO_0000115>A sum (district) of Omnogovi Province in southern Mongolia.</obo:IAO_0000115>
        <oboInOwl:hasOBONamespace>GAZ</oboInOwl:hasOBONamespace>
        <oboInOwl:id>GAZ:00027280</oboInOwl:id>
        <rdfs:label>Dalanzadgad District</rdfs:label>
    </owl:NamedIndividual>
    


    <!-- http://purl.obolibrary.org/obo/GAZ_00027281 -->

    <owl:NamedIndividual rdf:about="http://purl.obolibrary.org/obo/GAZ_00027281">
        <rdf:type rdf:resource="http://purl.obolibrary.org/obo/ENVO_00000004"/>
        <obo:RO_0001025 rdf:resource="http://purl.obolibrary.org/obo/GAZ_00014886"/>
        <obo:IAO_0000115>A sum (district) of Ovorkhangai Province in southern Mongolia.</obo:IAO_0000115>
        <oboInOwl:hasOBONamespace>GAZ</oboInOwl:hasOBONamespace>
        <oboInOwl:id>GAZ:00027281</oboInOwl:id>
        <rdfs:label>Sant District</rdfs:label>
    </owl:NamedIndividual>
    


    <!-- http://purl.obolibrary.org/obo/GAZ_00027282 -->

    <owl:NamedIndividual rdf:about="http://purl.obolibrary.org/obo/GAZ_00027282">
        <rdf:type rdf:resource="http://purl.obolibrary.org/obo/ENVO_00000004"/>
        <obo:RO_0001025 rdf:resource="http://purl.obolibrary.org/obo/GAZ_00014886"/>
        <obo:IAO_0000115>A sum (district) of Ovorkhangai Province in southern Mongolia.</obo:IAO_0000115>
        <oboInOwl:hasOBONamespace>GAZ</oboInOwl:hasOBONamespace>
        <oboInOwl:id>GAZ:00027282</oboInOwl:id>
        <rdfs:label>Nariinteel District</rdfs:label>
    </owl:NamedIndividual>
    


    <!-- http://purl.obolibrary.org/obo/GAZ_00027283 -->

    <owl:NamedIndividual rdf:about="http://purl.obolibrary.org/obo/GAZ_00027283">
        <rdf:type rdf:resource="http://purl.obolibrary.org/obo/ENVO_00000004"/>
        <obo:RO_0001025 rdf:resource="http://purl.obolibrary.org/obo/GAZ_00014886"/>
        <obo:IAO_0000115>A sum (district) of Ovorkhangai Province in southern Mongolia.</obo:IAO_0000115>
        <oboInOwl:hasOBONamespace>GAZ</oboInOwl:hasOBONamespace>
        <oboInOwl:id>GAZ:00027283</oboInOwl:id>
        <rdfs:label>Baruun Bayan-Ulaan District</rdfs:label>
    </owl:NamedIndividual>
    


    <!-- http://purl.obolibrary.org/obo/GAZ_00027284 -->

    <owl:NamedIndividual rdf:about="http://purl.obolibrary.org/obo/GAZ_00027284">
        <rdf:type rdf:resource="http://purl.obolibrary.org/obo/ENVO_00000004"/>
        <obo:RO_0001025 rdf:resource="http://purl.obolibrary.org/obo/GAZ_00014886"/>
        <obo:IAO_0000115>A sum (district) of Ovorkhangai Province in southern Mongolia.</obo:IAO_0000115>
        <oboInOwl:hasOBONamespace>GAZ</oboInOwl:hasOBONamespace>
        <oboInOwl:id>GAZ:00027284</oboInOwl:id>
        <rdfs:label>Bogd District</rdfs:label>
    </owl:NamedIndividual>
    


    <!-- http://purl.obolibrary.org/obo/GAZ_00027285 -->

    <owl:NamedIndividual rdf:about="http://purl.obolibrary.org/obo/GAZ_00027285">
        <rdf:type rdf:resource="http://purl.obolibrary.org/obo/ENVO_00000004"/>
        <obo:RO_0001025 rdf:resource="http://purl.obolibrary.org/obo/GAZ_00014886"/>
        <obo:IAO_0000115>A sum (district) of Ovorkhangai Province in southern Mongolia.</obo:IAO_0000115>
        <oboInOwl:hasOBONamespace>GAZ</oboInOwl:hasOBONamespace>
        <oboInOwl:id>GAZ:00027285</oboInOwl:id>
        <rdfs:label>Bayan-Ondor District</rdfs:label>
    </owl:NamedIndividual>
    


    <!-- http://purl.obolibrary.org/obo/GAZ_00027286 -->

    <owl:NamedIndividual rdf:about="http://purl.obolibrary.org/obo/GAZ_00027286">
        <rdf:type rdf:resource="http://purl.obolibrary.org/obo/ENVO_00000004"/>
        <obo:RO_0001025 rdf:resource="http://purl.obolibrary.org/obo/GAZ_00014886"/>
        <obo:IAO_0000115>A sum (district) of Ovorkhangai Province in southern Mongolia.</obo:IAO_0000115>
        <oboInOwl:hasOBONamespace>GAZ</oboInOwl:hasOBONamespace>
        <oboInOwl:id>GAZ:00027286</oboInOwl:id>
        <rdfs:label>Kharkhorin District</rdfs:label>
    </owl:NamedIndividual>
    


    <!-- http://purl.obolibrary.org/obo/GAZ_00027287 -->

    <owl:NamedIndividual rdf:about="http://purl.obolibrary.org/obo/GAZ_00027287">
        <rdf:type rdf:resource="http://purl.obolibrary.org/obo/ENVO_00000004"/>
        <obo:RO_0001025 rdf:resource="http://purl.obolibrary.org/obo/GAZ_00014886"/>
        <obo:IAO_0000115>A sum (district) of Ovorkhangai Province in southern Mongolia.</obo:IAO_0000115>
        <oboInOwl:hasOBONamespace>GAZ</oboInOwl:hasOBONamespace>
        <oboInOwl:id>GAZ:00027287</oboInOwl:id>
        <rdfs:label>Khairkhandulaan District</rdfs:label>
    </owl:NamedIndividual>
    


    <!-- http://purl.obolibrary.org/obo/GAZ_00027288 -->

    <owl:NamedIndividual rdf:about="http://purl.obolibrary.org/obo/GAZ_00027288">
        <rdf:type rdf:resource="http://purl.obolibrary.org/obo/ENVO_00000004"/>
        <obo:RO_0001025 rdf:resource="http://purl.obolibrary.org/obo/GAZ_00014882"/>
        <obo:IAO_0000115>A sum (district) of Omnogovi Province in southern Mongolia.</obo:IAO_0000115>
        <oboInOwl:hasOBONamespace>GAZ</oboInOwl:hasOBONamespace>
        <oboInOwl:id>GAZ:00027288</oboInOwl:id>
        <rdfs:label>Tsogt-Ovoo District</rdfs:label>
    </owl:NamedIndividual>
    


    <!-- http://purl.obolibrary.org/obo/GAZ_00027289 -->

    <owl:NamedIndividual rdf:about="http://purl.obolibrary.org/obo/GAZ_00027289">
        <rdf:type rdf:resource="http://purl.obolibrary.org/obo/ENVO_00000004"/>
        <obo:RO_0001025 rdf:resource="http://purl.obolibrary.org/obo/GAZ_00014884"/>
        <obo:IAO_0000115>A sum (district) of Orkhon Province in northern Mongolia.</obo:IAO_0000115>
        <oboInOwl:hasOBONamespace>GAZ</oboInOwl:hasOBONamespace>
        <oboInOwl:id>GAZ:00027289</oboInOwl:id>
        <rdfs:label>Jargalant District</rdfs:label>
    </owl:NamedIndividual>
    


    <!-- http://purl.obolibrary.org/obo/GAZ_00027290 -->

    <owl:NamedIndividual rdf:about="http://purl.obolibrary.org/obo/GAZ_00027290">
        <rdf:type rdf:resource="http://purl.obolibrary.org/obo/ENVO_00000004"/>
        <obo:RO_0001025 rdf:resource="http://purl.obolibrary.org/obo/GAZ_00014882"/>
        <obo:IAO_0000115>A sum (district) of Omnogovi Province in southern Mongolia.</obo:IAO_0000115>
        <oboInOwl:hasOBONamespace>GAZ</oboInOwl:hasOBONamespace>
        <oboInOwl:id>GAZ:00027290</oboInOwl:id>
        <rdfs:label>Manlai District</rdfs:label>
    </owl:NamedIndividual>
    


    <!-- http://purl.obolibrary.org/obo/GAZ_00027291 -->

    <owl:NamedIndividual rdf:about="http://purl.obolibrary.org/obo/GAZ_00027291">
        <rdf:type rdf:resource="http://purl.obolibrary.org/obo/ENVO_00000004"/>
        <obo:RO_0001025 rdf:resource="http://purl.obolibrary.org/obo/GAZ_00014886"/>
        <obo:IAO_0000115>A sum (district) of Ovorkhangai Province in southern Mongolia.</obo:IAO_0000115>
        <oboInOwl:hasOBONamespace>GAZ</oboInOwl:hasOBONamespace>
        <oboInOwl:id>GAZ:00027291</oboInOwl:id>
        <rdfs:label>Bayangol District</rdfs:label>
    </owl:NamedIndividual>
    


    <!-- http://purl.obolibrary.org/obo/GAZ_00027292 -->

    <owl:NamedIndividual rdf:about="http://purl.obolibrary.org/obo/GAZ_00027292">
        <rdf:type rdf:resource="http://purl.obolibrary.org/obo/ENVO_00000004"/>
        <obo:RO_0001025 rdf:resource="http://purl.obolibrary.org/obo/GAZ_00014882"/>
        <obo:IAO_0000115>A sum (district) of Omnogovi Province in southern Mongolia.</obo:IAO_0000115>
        <oboInOwl:hasOBONamespace>GAZ</oboInOwl:hasOBONamespace>
        <oboInOwl:id>GAZ:00027292</oboInOwl:id>
        <rdfs:label>Tsogttsetsii District</rdfs:label>
    </owl:NamedIndividual>
    


    <!-- http://purl.obolibrary.org/obo/GAZ_00027293 -->

    <owl:NamedIndividual rdf:about="http://purl.obolibrary.org/obo/GAZ_00027293">
        <rdf:type rdf:resource="http://purl.obolibrary.org/obo/ENVO_00000004"/>
        <obo:RO_0001025 rdf:resource="http://purl.obolibrary.org/obo/GAZ_00014886"/>
        <obo:IAO_0000115>A sum (district) of Ovorkhangai Province in southern Mongolia.</obo:IAO_0000115>
        <oboInOwl:hasOBONamespace>GAZ</oboInOwl:hasOBONamespace>
        <oboInOwl:id>GAZ:00027293</oboInOwl:id>
        <rdfs:label>Zuunbayan-Ulaan District</rdfs:label>
    </owl:NamedIndividual>
    


    <!-- http://purl.obolibrary.org/obo/GAZ_00027294 -->

    <owl:NamedIndividual rdf:about="http://purl.obolibrary.org/obo/GAZ_00027294">
        <rdf:type rdf:resource="http://purl.obolibrary.org/obo/ENVO_00000004"/>
        <obo:RO_0001025 rdf:resource="http://purl.obolibrary.org/obo/GAZ_00014886"/>
        <obo:IAO_0000115>A sum (district) of Ovorkhangai Province in southern Mongolia.</obo:IAO_0000115>
        <oboInOwl:hasOBONamespace>GAZ</oboInOwl:hasOBONamespace>
        <oboInOwl:id>GAZ:00027294</oboInOwl:id>
        <rdfs:label>Uyanga District</rdfs:label>
    </owl:NamedIndividual>
    


    <!-- http://purl.obolibrary.org/obo/GAZ_00027295 -->

    <owl:NamedIndividual rdf:about="http://purl.obolibrary.org/obo/GAZ_00027295">
        <rdf:type rdf:resource="http://purl.obolibrary.org/obo/ENVO_00000004"/>
        <obo:RO_0001025 rdf:resource="http://purl.obolibrary.org/obo/GAZ_00014886"/>
        <obo:IAO_0000115>A sum (district) of Ovorkhangai Province in southern Mongolia.</obo:IAO_0000115>
        <oboInOwl:hasOBONamespace>GAZ</oboInOwl:hasOBONamespace>
        <oboInOwl:id>GAZ:00027295</oboInOwl:id>
        <rdfs:label>Yesonzuil District</rdfs:label>
    </owl:NamedIndividual>
    


    <!-- http://purl.obolibrary.org/obo/GAZ_00027296 -->

    <owl:NamedIndividual rdf:about="http://purl.obolibrary.org/obo/GAZ_00027296">
        <rdf:type rdf:resource="http://purl.obolibrary.org/obo/ENVO_00000004"/>
        <obo:RO_0001025 rdf:resource="http://purl.obolibrary.org/obo/GAZ_00014881"/>
        <obo:IAO_0000115>A sum (district) of Selenge Province in northern Mongolia.</obo:IAO_0000115>
        <oboInOwl:hasOBONamespace>GAZ</oboInOwl:hasOBONamespace>
        <oboInOwl:id>GAZ:00027296</oboInOwl:id>
        <rdfs:label>Tushig District</rdfs:label>
    </owl:NamedIndividual>
    


    <!-- http://purl.obolibrary.org/obo/GAZ_00027297 -->

    <owl:NamedIndividual rdf:about="http://purl.obolibrary.org/obo/GAZ_00027297">
        <rdf:type rdf:resource="http://purl.obolibrary.org/obo/ENVO_00000004"/>
        <obo:RO_0001025 rdf:resource="http://purl.obolibrary.org/obo/GAZ_00014887"/>
        <obo:IAO_0000115>A sum (district) of Sukhbaatar Province in eastern Mongolia.</obo:IAO_0000115>
        <oboInOwl:hasOBONamespace>GAZ</oboInOwl:hasOBONamespace>
        <oboInOwl:id>GAZ:00027297</oboInOwl:id>
        <rdfs:label>Khalzan District</rdfs:label>
    </owl:NamedIndividual>
    


    <!-- http://purl.obolibrary.org/obo/GAZ_00027298 -->

    <owl:NamedIndividual rdf:about="http://purl.obolibrary.org/obo/GAZ_00027298">
        <rdf:type rdf:resource="http://purl.obolibrary.org/obo/ENVO_00000004"/>
        <obo:RO_0001025 rdf:resource="http://purl.obolibrary.org/obo/GAZ_00014881"/>
        <obo:IAO_0000115>A sum (district) of Selenge Province in northern Mongolia.</obo:IAO_0000115>
        <oboInOwl:hasOBONamespace>GAZ</oboInOwl:hasOBONamespace>
        <oboInOwl:id>GAZ:00027298</oboInOwl:id>
        <rdfs:label>Altanbulag District</rdfs:label>
    </owl:NamedIndividual>
    


    <!-- http://purl.obolibrary.org/obo/GAZ_00027299 -->

    <owl:NamedIndividual rdf:about="http://purl.obolibrary.org/obo/GAZ_00027299">
        <rdf:type rdf:resource="http://purl.obolibrary.org/obo/ENVO_00000004"/>
        <obo:RO_0001025 rdf:resource="http://purl.obolibrary.org/obo/GAZ_00014887"/>
        <obo:IAO_0000115>A sum (district) of Sukhbaatar Province in eastern Mongolia.</obo:IAO_0000115>
        <oboInOwl:hasOBONamespace>GAZ</oboInOwl:hasOBONamespace>
        <oboInOwl:id>GAZ:00027299</oboInOwl:id>
        <rdfs:label>Sukhbaatar District</rdfs:label>
    </owl:NamedIndividual>
    


    <!-- http://purl.obolibrary.org/obo/GAZ_00027300 -->

    <owl:NamedIndividual rdf:about="http://purl.obolibrary.org/obo/GAZ_00027300">
        <rdf:type rdf:resource="http://purl.obolibrary.org/obo/ENVO_00000004"/>
        <obo:RO_0001025 rdf:resource="http://purl.obolibrary.org/obo/GAZ_00014887"/>
        <obo:IAO_0000115>A sum (district) of Sukhbaatar Province in eastern Mongolia.</obo:IAO_0000115>
        <oboInOwl:hasOBONamespace>GAZ</oboInOwl:hasOBONamespace>
        <oboInOwl:id>GAZ:00027300</oboInOwl:id>
        <rdfs:label>Monkhkhaan District</rdfs:label>
    </owl:NamedIndividual>
    


    <!-- http://purl.obolibrary.org/obo/GAZ_00027301 -->

    <owl:NamedIndividual rdf:about="http://purl.obolibrary.org/obo/GAZ_00027301">
        <rdf:type rdf:resource="http://purl.obolibrary.org/obo/ENVO_00000004"/>
        <obo:RO_0001025 rdf:resource="http://purl.obolibrary.org/obo/GAZ_00014881"/>
        <obo:IAO_0000115>A sum (district) of Selenge Province in northern Mongolia.</obo:IAO_0000115>
        <oboInOwl:hasOBONamespace>GAZ</oboInOwl:hasOBONamespace>
        <oboInOwl:id>GAZ:00027301</oboInOwl:id>
        <rdfs:label>Tsagaannuur District</rdfs:label>
    </owl:NamedIndividual>
    


    <!-- http://purl.obolibrary.org/obo/GAZ_00027302 -->

    <owl:NamedIndividual rdf:about="http://purl.obolibrary.org/obo/GAZ_00027302">
        <rdf:type rdf:resource="http://purl.obolibrary.org/obo/ENVO_00000004"/>
        <obo:RO_0001025 rdf:resource="http://purl.obolibrary.org/obo/GAZ_00014887"/>
        <obo:IAO_0000115>A sum (district) of Sukhbaatar Province in eastern Mongolia.</obo:IAO_0000115>
        <oboInOwl:hasOBONamespace>GAZ</oboInOwl:hasOBONamespace>
        <oboInOwl:id>GAZ:00027302</oboInOwl:id>
        <rdfs:label>Bayandelger District</rdfs:label>
    </owl:NamedIndividual>
    


    <!-- http://purl.obolibrary.org/obo/GAZ_00027303 -->

    <owl:NamedIndividual rdf:about="http://purl.obolibrary.org/obo/GAZ_00027303">
        <rdf:type rdf:resource="http://purl.obolibrary.org/obo/ENVO_00000004"/>
        <obo:RO_0001025 rdf:resource="http://purl.obolibrary.org/obo/GAZ_00014881"/>
        <obo:IAO_0000115>A sum (district) of Selenge Province in northern Mongolia.</obo:IAO_0000115>
        <oboInOwl:hasOBONamespace>GAZ</oboInOwl:hasOBONamespace>
        <oboInOwl:id>GAZ:00027303</oboInOwl:id>
        <rdfs:label>Orkhontuul District</rdfs:label>
    </owl:NamedIndividual>
    


    <!-- http://purl.obolibrary.org/obo/GAZ_00027304 -->

    <owl:NamedIndividual rdf:about="http://purl.obolibrary.org/obo/GAZ_00027304">
        <rdf:type rdf:resource="http://purl.obolibrary.org/obo/ENVO_00000004"/>
        <obo:RO_0001025 rdf:resource="http://purl.obolibrary.org/obo/GAZ_00014887"/>
        <obo:IAO_0000115>A sum (district) of Sukhbaatar Province in eastern Mongolia.</obo:IAO_0000115>
        <oboInOwl:hasOBONamespace>GAZ</oboInOwl:hasOBONamespace>
        <oboInOwl:id>GAZ:00027304</oboInOwl:id>
        <rdfs:label>Tuvshinshiree District</rdfs:label>
    </owl:NamedIndividual>
    


    <!-- http://purl.obolibrary.org/obo/GAZ_00027305 -->

    <owl:NamedIndividual rdf:about="http://purl.obolibrary.org/obo/GAZ_00027305">
        <rdf:type rdf:resource="http://purl.obolibrary.org/obo/ENVO_00000004"/>
        <obo:RO_0001025 rdf:resource="http://purl.obolibrary.org/obo/GAZ_00014881"/>
        <obo:IAO_0000115>A sum (district) of Selenge Province in northern Mongolia.</obo:IAO_0000115>
        <oboInOwl:hasOBONamespace>GAZ</oboInOwl:hasOBONamespace>
        <oboInOwl:id>GAZ:00027305</oboInOwl:id>
        <rdfs:label>Orkhon District</rdfs:label>
    </owl:NamedIndividual>
    


    <!-- http://purl.obolibrary.org/obo/GAZ_00027306 -->

    <owl:NamedIndividual rdf:about="http://purl.obolibrary.org/obo/GAZ_00027306">
        <rdf:type rdf:resource="http://purl.obolibrary.org/obo/ENVO_00000004"/>
        <obo:RO_0001025 rdf:resource="http://purl.obolibrary.org/obo/GAZ_00014887"/>
        <obo:IAO_0000115>A sum (district) of Sukhbaatar Province in eastern Mongolia.</obo:IAO_0000115>
        <oboInOwl:hasOBONamespace>GAZ</oboInOwl:hasOBONamespace>
        <oboInOwl:id>GAZ:00027306</oboInOwl:id>
        <rdfs:label>Erdenetsagaan District</rdfs:label>
    </owl:NamedIndividual>
    


    <!-- http://purl.obolibrary.org/obo/GAZ_00027307 -->

    <owl:NamedIndividual rdf:about="http://purl.obolibrary.org/obo/GAZ_00027307">
        <rdf:type rdf:resource="http://purl.obolibrary.org/obo/ENVO_00000004"/>
        <obo:RO_0001025 rdf:resource="http://purl.obolibrary.org/obo/GAZ_00014881"/>
        <obo:IAO_0000115>A sum (district) of Selenge Province in northern Mongolia.</obo:IAO_0000115>
        <oboInOwl:hasOBONamespace>GAZ</oboInOwl:hasOBONamespace>
        <oboInOwl:id>GAZ:00027307</oboInOwl:id>
        <rdfs:label>Zuunburen District</rdfs:label>
    </owl:NamedIndividual>
    


    <!-- http://purl.obolibrary.org/obo/GAZ_00027308 -->

    <owl:NamedIndividual rdf:about="http://purl.obolibrary.org/obo/GAZ_00027308">
        <rdf:type rdf:resource="http://purl.obolibrary.org/obo/ENVO_00000004"/>
        <obo:RO_0001025 rdf:resource="http://purl.obolibrary.org/obo/GAZ_00014887"/>
        <obo:IAO_0000115>A sum (district) of Sukhbaatar Province in eastern Mongolia.</obo:IAO_0000115>
        <oboInOwl:hasOBONamespace>GAZ</oboInOwl:hasOBONamespace>
        <oboInOwl:id>GAZ:00027308</oboInOwl:id>
        <rdfs:label>Dariganga District</rdfs:label>
    </owl:NamedIndividual>
    


    <!-- http://purl.obolibrary.org/obo/GAZ_00027309 -->

    <owl:NamedIndividual rdf:about="http://purl.obolibrary.org/obo/GAZ_00027309">
        <rdf:type rdf:resource="http://purl.obolibrary.org/obo/ENVO_00000004"/>
        <obo:RO_0001025 rdf:resource="http://purl.obolibrary.org/obo/GAZ_00014881"/>
        <obo:IAO_0000115>A sum (district) of Selenge Province in northern Mongolia.</obo:IAO_0000115>
        <oboInOwl:hasOBONamespace>GAZ</oboInOwl:hasOBONamespace>
        <oboInOwl:id>GAZ:00027309</oboInOwl:id>
        <rdfs:label>Mandal District</rdfs:label>
    </owl:NamedIndividual>
    


    <!-- http://purl.obolibrary.org/obo/GAZ_00027310 -->

    <owl:NamedIndividual rdf:about="http://purl.obolibrary.org/obo/GAZ_00027310">
        <rdf:type rdf:resource="http://purl.obolibrary.org/obo/ENVO_00000004"/>
        <obo:RO_0001025 rdf:resource="http://purl.obolibrary.org/obo/GAZ_00014887"/>
        <obo:IAO_0000115>A sum (district) of Sukhbaatar Province in eastern Mongolia.</obo:IAO_0000115>
        <oboInOwl:hasOBONamespace>GAZ</oboInOwl:hasOBONamespace>
        <oboInOwl:id>GAZ:00027310</oboInOwl:id>
        <rdfs:label>Tumentsogt District</rdfs:label>
    </owl:NamedIndividual>
    


    <!-- http://purl.obolibrary.org/obo/GAZ_00027311 -->

    <owl:NamedIndividual rdf:about="http://purl.obolibrary.org/obo/GAZ_00027311">
        <rdf:type rdf:resource="http://purl.obolibrary.org/obo/ENVO_00000004"/>
        <obo:RO_0001025 rdf:resource="http://purl.obolibrary.org/obo/GAZ_00014881"/>
        <obo:IAO_0000115>A sum (district) of Selenge Province in northern Mongolia.</obo:IAO_0000115>
        <oboInOwl:hasOBONamespace>GAZ</oboInOwl:hasOBONamespace>
        <oboInOwl:id>GAZ:00027311</oboInOwl:id>
        <rdfs:label>Yeroo District</rdfs:label>
    </owl:NamedIndividual>
    


    <!-- http://purl.obolibrary.org/obo/GAZ_00027312 -->

    <owl:NamedIndividual rdf:about="http://purl.obolibrary.org/obo/GAZ_00027312">
        <rdf:type rdf:resource="http://purl.obolibrary.org/obo/ENVO_00000004"/>
        <obo:RO_0001025 rdf:resource="http://purl.obolibrary.org/obo/GAZ_00014887"/>
        <obo:IAO_0000115>A sum (district) of Sukhbaatar Province in eastern Mongolia.</obo:IAO_0000115>
        <oboInOwl:hasOBONamespace>GAZ</oboInOwl:hasOBONamespace>
        <oboInOwl:id>GAZ:00027312</oboInOwl:id>
        <rdfs:label>Ongon District</rdfs:label>
    </owl:NamedIndividual>
    


    <!-- http://purl.obolibrary.org/obo/GAZ_00027313 -->

    <owl:NamedIndividual rdf:about="http://purl.obolibrary.org/obo/GAZ_00027313">
        <rdf:type rdf:resource="http://purl.obolibrary.org/obo/ENVO_00000004"/>
        <obo:RO_0001025 rdf:resource="http://purl.obolibrary.org/obo/GAZ_00014887"/>
        <obo:IAO_0000115>A sum (district) of Sukhbaatar Province in eastern Mongolia.</obo:IAO_0000115>
        <oboInOwl:hasOBONamespace>GAZ</oboInOwl:hasOBONamespace>
        <oboInOwl:id>GAZ:00027313</oboInOwl:id>
        <rdfs:label>Uulbayan District</rdfs:label>
    </owl:NamedIndividual>
    


    <!-- http://purl.obolibrary.org/obo/GAZ_00027314 -->

    <owl:NamedIndividual rdf:about="http://purl.obolibrary.org/obo/GAZ_00027314">
        <rdf:type rdf:resource="http://purl.obolibrary.org/obo/ENVO_00000004"/>
        <obo:RO_0001025 rdf:resource="http://purl.obolibrary.org/obo/GAZ_00014881"/>
        <obo:IAO_0000115>A sum (district) of Selenge Province in northern Mongolia.</obo:IAO_0000115>
        <oboInOwl:hasOBONamespace>GAZ</oboInOwl:hasOBONamespace>
        <oboInOwl:id>GAZ:00027314</oboInOwl:id>
        <rdfs:label>Sant District</rdfs:label>
    </owl:NamedIndividual>
    


    <!-- http://purl.obolibrary.org/obo/GAZ_00027315 -->

    <owl:NamedIndividual rdf:about="http://purl.obolibrary.org/obo/GAZ_00027315">
        <rdf:type rdf:resource="http://purl.obolibrary.org/obo/ENVO_00000004"/>
        <obo:RO_0001025 rdf:resource="http://purl.obolibrary.org/obo/GAZ_00014881"/>
        <obo:IAO_0000115>A sum (district) of Selenge Province in northern Mongolia.</obo:IAO_0000115>
        <oboInOwl:hasOBONamespace>GAZ</oboInOwl:hasOBONamespace>
        <oboInOwl:id>GAZ:00027315</oboInOwl:id>
        <rdfs:label>Javkhlant District</rdfs:label>
    </owl:NamedIndividual>
    


    <!-- http://purl.obolibrary.org/obo/GAZ_00027316 -->

    <owl:NamedIndividual rdf:about="http://purl.obolibrary.org/obo/GAZ_00027316">
        <rdf:type rdf:resource="http://purl.obolibrary.org/obo/ENVO_00000004"/>
        <obo:RO_0001025 rdf:resource="http://purl.obolibrary.org/obo/GAZ_00014881"/>
        <obo:IAO_0000115>A sum (district) of Selenge Province in northern Mongolia. The capital of Selenge Province in northern Mongolia, on the Orkhon river.</obo:IAO_0000115>
        <oboInOwl:hasOBONamespace>GAZ</oboInOwl:hasOBONamespace>
        <oboInOwl:id>GAZ:00027316</oboInOwl:id>
        <rdfs:label>Sukhbaatar City</rdfs:label>
    </owl:NamedIndividual>
    


    <!-- http://purl.obolibrary.org/obo/GAZ_00027317 -->

    <owl:NamedIndividual rdf:about="http://purl.obolibrary.org/obo/GAZ_00027317">
        <rdf:type rdf:resource="http://purl.obolibrary.org/obo/ENVO_00000004"/>
        <obo:RO_0001025 rdf:resource="http://purl.obolibrary.org/obo/GAZ_00014881"/>
        <obo:IAO_0000115>A sum (district) of Selenge Province in northern Mongolia.</obo:IAO_0000115>
        <oboInOwl:hasOBONamespace>GAZ</oboInOwl:hasOBONamespace>
        <oboInOwl:id>GAZ:00027317</oboInOwl:id>
        <rdfs:label>Khushaat District</rdfs:label>
    </owl:NamedIndividual>
    


    <!-- http://purl.obolibrary.org/obo/GAZ_00027318 -->

    <owl:NamedIndividual rdf:about="http://purl.obolibrary.org/obo/GAZ_00027318">
        <rdf:type rdf:resource="http://purl.obolibrary.org/obo/ENVO_00000004"/>
        <obo:RO_0001025 rdf:resource="http://purl.obolibrary.org/obo/GAZ_00014881"/>
        <obo:IAO_0000115>A sum (district) of Selenge Province in northern Mongolia.</obo:IAO_0000115>
        <oboInOwl:hasOBONamespace>GAZ</oboInOwl:hasOBONamespace>
        <oboInOwl:id>GAZ:00027318</oboInOwl:id>
        <rdfs:label>Saykhan District</rdfs:label>
    </owl:NamedIndividual>
    


    <!-- http://purl.obolibrary.org/obo/GAZ_00027319 -->

    <owl:NamedIndividual rdf:about="http://purl.obolibrary.org/obo/GAZ_00027319">
        <rdf:type rdf:resource="http://purl.obolibrary.org/obo/ENVO_00000004"/>
        <obo:RO_0001025 rdf:resource="http://purl.obolibrary.org/obo/GAZ_00014881"/>
        <obo:IAO_0000115>A sum (district) of Selenge Province in northern Mongolia.</obo:IAO_0000115>
        <oboInOwl:hasOBONamespace>GAZ</oboInOwl:hasOBONamespace>
        <oboInOwl:id>GAZ:00027319</oboInOwl:id>
        <rdfs:label>Bayangol District</rdfs:label>
    </owl:NamedIndividual>
    


    <!-- http://purl.obolibrary.org/obo/GAZ_00027320 -->

    <owl:NamedIndividual rdf:about="http://purl.obolibrary.org/obo/GAZ_00027320">
        <rdf:type rdf:resource="http://purl.obolibrary.org/obo/ENVO_00000004"/>
        <obo:RO_0001025 rdf:resource="http://purl.obolibrary.org/obo/GAZ_00014881"/>
        <obo:IAO_0000115>A sum (district) of Selenge Province in northern Mongolia.</obo:IAO_0000115>
        <oboInOwl:hasOBONamespace>GAZ</oboInOwl:hasOBONamespace>
        <oboInOwl:id>GAZ:00027320</oboInOwl:id>
        <rdfs:label>Khuder District</rdfs:label>
    </owl:NamedIndividual>
    


    <!-- http://purl.obolibrary.org/obo/GAZ_00027321 -->

    <owl:NamedIndividual rdf:about="http://purl.obolibrary.org/obo/GAZ_00027321">
        <rdf:type rdf:resource="http://purl.obolibrary.org/obo/ENVO_00000004"/>
        <obo:RO_0001025 rdf:resource="http://purl.obolibrary.org/obo/GAZ_00014887"/>
        <obo:IAO_0000115>A sum (district) of Sukhbaatar Province in eastern Mongolia.</obo:IAO_0000115>
        <oboInOwl:hasOBONamespace>GAZ</oboInOwl:hasOBONamespace>
        <oboInOwl:id>GAZ:00027321</oboInOwl:id>
        <rdfs:label>Naran District</rdfs:label>
    </owl:NamedIndividual>
    


    <!-- http://purl.obolibrary.org/obo/GAZ_00027322 -->

    <owl:NamedIndividual rdf:about="http://purl.obolibrary.org/obo/GAZ_00027322">
        <rdf:type rdf:resource="http://purl.obolibrary.org/obo/ENVO_00000004"/>
        <obo:RO_0001025 rdf:resource="http://purl.obolibrary.org/obo/GAZ_00014881"/>
        <obo:IAO_0000115>A sum (district) of Selenge Province in northern Mongolia.</obo:IAO_0000115>
        <oboInOwl:hasOBONamespace>GAZ</oboInOwl:hasOBONamespace>
        <oboInOwl:id>GAZ:00027322</oboInOwl:id>
        <rdfs:label>Shaamar District</rdfs:label>
    </owl:NamedIndividual>
    


    <!-- http://purl.obolibrary.org/obo/GAZ_00027323 -->

    <owl:NamedIndividual rdf:about="http://purl.obolibrary.org/obo/GAZ_00027323">
        <rdf:type rdf:resource="http://purl.obolibrary.org/obo/ENVO_00000004"/>
        <obo:RO_0001025 rdf:resource="http://purl.obolibrary.org/obo/GAZ_00014881"/>
        <obo:IAO_0000115>A sum (district) of Selenge Province in northern Mongolia.</obo:IAO_0000115>
        <oboInOwl:hasOBONamespace>GAZ</oboInOwl:hasOBONamespace>
        <oboInOwl:id>GAZ:00027323</oboInOwl:id>
        <rdfs:label>Baruunburen District</rdfs:label>
    </owl:NamedIndividual>
    


    <!-- http://purl.obolibrary.org/obo/GAZ_00027324 -->

    <owl:NamedIndividual rdf:about="http://purl.obolibrary.org/obo/GAZ_00027324">
        <obo:RO_0001025 rdf:resource="http://purl.obolibrary.org/obo/GAZ_00014887"/>
        <obo:IAO_0000115>A sum in eastern Mongolia and the capital of Sukhbaatar Province. It is an enclave in the surrounding Sukhbaatar sum.</obo:IAO_0000115>
        <oboInOwl:hasOBONamespace>GAZ</oboInOwl:hasOBONamespace>
        <oboInOwl:id>GAZ:00027324</oboInOwl:id>
        <rdfs:label>Baruun-Urt District</rdfs:label>
    </owl:NamedIndividual>
    


    <!-- http://purl.obolibrary.org/obo/GAZ_00027325 -->

    <owl:NamedIndividual rdf:about="http://purl.obolibrary.org/obo/GAZ_00027325">
        <rdf:type rdf:resource="http://purl.obolibrary.org/obo/ENVO_00000004"/>
        <obo:RO_0001025 rdf:resource="http://purl.obolibrary.org/obo/GAZ_00014887"/>
        <obo:IAO_0000115>A sum (district) of Sukhbaatar Province in eastern Mongolia.</obo:IAO_0000115>
        <oboInOwl:hasOBONamespace>GAZ</oboInOwl:hasOBONamespace>
        <oboInOwl:id>GAZ:00027325</oboInOwl:id>
        <rdfs:label>Asgat District</rdfs:label>
    </owl:NamedIndividual>
    


    <!-- http://purl.obolibrary.org/obo/GAZ_00027326 -->

    <owl:NamedIndividual rdf:about="http://purl.obolibrary.org/obo/GAZ_00027326">
        <rdf:type rdf:resource="http://purl.obolibrary.org/obo/ENVO_00000004"/>
        <obo:RO_0001025 rdf:resource="http://purl.obolibrary.org/obo/GAZ_00117540"/>
        <obo:IAO_0000115>A sum (district) of Uvs Province in Mongolia.</obo:IAO_0000115>
        <oboInOwl:hasOBONamespace>GAZ</oboInOwl:hasOBONamespace>
        <oboInOwl:id>GAZ:00027326</oboInOwl:id>
        <rdfs:label>Khovd District</rdfs:label>
    </owl:NamedIndividual>
    


    <!-- http://purl.obolibrary.org/obo/GAZ_00027327 -->

    <owl:NamedIndividual rdf:about="http://purl.obolibrary.org/obo/GAZ_00027327">
        <rdf:type rdf:resource="http://purl.obolibrary.org/obo/ENVO_00000004"/>
        <obo:RO_0001025 rdf:resource="http://purl.obolibrary.org/obo/GAZ_00014876"/>
        <obo:IAO_0000115>A sum (district) of Uvs Province in Mongolia.</obo:IAO_0000115>
        <oboInOwl:hasOBONamespace>GAZ</oboInOwl:hasOBONamespace>
        <oboInOwl:id>GAZ:00027327</oboInOwl:id>
        <rdfs:label>Khyargas District</rdfs:label>
    </owl:NamedIndividual>
    


    <!-- http://purl.obolibrary.org/obo/GAZ_00027328 -->

    <owl:NamedIndividual rdf:about="http://purl.obolibrary.org/obo/GAZ_00027328">
        <rdf:type rdf:resource="http://purl.obolibrary.org/obo/ENVO_00000004"/>
        <obo:RO_0001025 rdf:resource="http://purl.obolibrary.org/obo/GAZ_00014869"/>
        <obo:IAO_0000115>A sum (district) of Tov Province in Mongolia.</obo:IAO_0000115>
        <oboInOwl:hasOBONamespace>GAZ</oboInOwl:hasOBONamespace>
        <oboInOwl:id>GAZ:00027328</oboInOwl:id>
        <rdfs:label>Zuunmod District</rdfs:label>
    </owl:NamedIndividual>
    


    <!-- http://purl.obolibrary.org/obo/GAZ_00027329 -->

    <owl:NamedIndividual rdf:about="http://purl.obolibrary.org/obo/GAZ_00027329">
        <rdf:type rdf:resource="http://purl.obolibrary.org/obo/ENVO_00000004"/>
        <obo:RO_0001025 rdf:resource="http://purl.obolibrary.org/obo/GAZ_00117540"/>
        <obo:IAO_0000115>A sum (district) of Uvs Province in Mongolia. The sum is on the border of Mongolia and Russia; in the west it borders to Bayan-Olgii Province.</obo:IAO_0000115>
        <oboInOwl:hasOBONamespace>GAZ</oboInOwl:hasOBONamespace>
        <oboInOwl:id>GAZ:00027329</oboInOwl:id>
        <rdfs:label>Bokhmoron District</rdfs:label>
    </owl:NamedIndividual>
    


    <!-- http://purl.obolibrary.org/obo/GAZ_00027330 -->

    <owl:NamedIndividual rdf:about="http://purl.obolibrary.org/obo/GAZ_00027330">
        <rdf:type rdf:resource="http://purl.obolibrary.org/obo/ENVO_00000004"/>
        <obo:RO_0001025 rdf:resource="http://purl.obolibrary.org/obo/GAZ_00014876"/>
        <obo:IAO_0000115>A sum (district) of Uvs Province in Mongolia.</obo:IAO_0000115>
        <oboInOwl:hasOBONamespace>GAZ</oboInOwl:hasOBONamespace>
        <oboInOwl:id>GAZ:00027330</oboInOwl:id>
        <rdfs:label>Malchin District</rdfs:label>
    </owl:NamedIndividual>
    


    <!-- http://purl.obolibrary.org/obo/GAZ_00027331 -->

    <owl:NamedIndividual rdf:about="http://purl.obolibrary.org/obo/GAZ_00027331">
        <rdf:type rdf:resource="http://purl.obolibrary.org/obo/ENVO_00000004"/>
        <obo:RO_0001025 rdf:resource="http://purl.obolibrary.org/obo/GAZ_00014869"/>
        <obo:IAO_0000115>A sum (district) of Tov Province in Mongolia.</obo:IAO_0000115>
        <oboInOwl:hasOBONamespace>GAZ</oboInOwl:hasOBONamespace>
        <oboInOwl:id>GAZ:00027331</oboInOwl:id>
        <rdfs:label>Bayan District</rdfs:label>
    </owl:NamedIndividual>
    


    <!-- http://purl.obolibrary.org/obo/GAZ_00027332 -->

    <owl:NamedIndividual rdf:about="http://purl.obolibrary.org/obo/GAZ_00027332">
        <rdf:type rdf:resource="http://purl.obolibrary.org/obo/ENVO_00000004"/>
        <obo:RO_0001025 rdf:resource="http://purl.obolibrary.org/obo/GAZ_00014876"/>
        <obo:IAO_0000115>A sum (district) of Uvs Province in Mongolia.</obo:IAO_0000115>
        <oboInOwl:hasOBONamespace>GAZ</oboInOwl:hasOBONamespace>
        <oboInOwl:id>GAZ:00027332</oboInOwl:id>
        <rdfs:label>Davst District</rdfs:label>
    </owl:NamedIndividual>
    


    <!-- http://purl.obolibrary.org/obo/GAZ_00027333 -->

    <owl:NamedIndividual rdf:about="http://purl.obolibrary.org/obo/GAZ_00027333">
        <rdf:type rdf:resource="http://purl.obolibrary.org/obo/ENVO_00000004"/>
        <obo:RO_0001025 rdf:resource="http://purl.obolibrary.org/obo/GAZ_00014869"/>
        <obo:IAO_0000115>A sum (district) of Tov Province in Mongolia.</obo:IAO_0000115>
        <oboInOwl:hasOBONamespace>GAZ</oboInOwl:hasOBONamespace>
        <oboInOwl:id>GAZ:00027333</oboInOwl:id>
        <rdfs:label>Bayanchandmani District</rdfs:label>
    </owl:NamedIndividual>
    


    <!-- http://purl.obolibrary.org/obo/GAZ_00027334 -->

    <owl:NamedIndividual rdf:about="http://purl.obolibrary.org/obo/GAZ_00027334">
        <rdf:type rdf:resource="http://purl.obolibrary.org/obo/ENVO_00000004"/>
        <obo:RO_0001025 rdf:resource="http://purl.obolibrary.org/obo/GAZ_00014869"/>
        <obo:IAO_0000115>A sum (district) of Tov Province in Mongolia.</obo:IAO_0000115>
        <oboInOwl:hasOBONamespace>GAZ</oboInOwl:hasOBONamespace>
        <oboInOwl:id>GAZ:00027334</oboInOwl:id>
        <rdfs:label>Batsumber District</rdfs:label>
    </owl:NamedIndividual>
    


    <!-- http://purl.obolibrary.org/obo/GAZ_00027335 -->

    <owl:NamedIndividual rdf:about="http://purl.obolibrary.org/obo/GAZ_00027335">
        <rdf:type rdf:resource="http://purl.obolibrary.org/obo/ENVO_00000004"/>
        <obo:RO_0001025 rdf:resource="http://purl.obolibrary.org/obo/GAZ_00014869"/>
        <obo:IAO_0000115>A sum (district) of Tov Province in Mongolia.</obo:IAO_0000115>
        <oboInOwl:hasOBONamespace>GAZ</oboInOwl:hasOBONamespace>
        <oboInOwl:id>GAZ:00027335</oboInOwl:id>
        <rdfs:label>Bomuur District</rdfs:label>
    </owl:NamedIndividual>
    


    <!-- http://purl.obolibrary.org/obo/GAZ_00027336 -->

    <owl:NamedIndividual rdf:about="http://purl.obolibrary.org/obo/GAZ_00027336">
        <rdf:type rdf:resource="http://purl.obolibrary.org/obo/ENVO_00000004"/>
        <obo:RO_0001025 rdf:resource="http://purl.obolibrary.org/obo/GAZ_00014869"/>
        <obo:IAO_0000115>A sum (district) of Tov Province in Mongolia.</obo:IAO_0000115>
        <oboInOwl:hasOBONamespace>GAZ</oboInOwl:hasOBONamespace>
        <oboInOwl:id>GAZ:00027336</oboInOwl:id>
        <rdfs:label>Bayantsogt District</rdfs:label>
    </owl:NamedIndividual>
    


    <!-- http://purl.obolibrary.org/obo/GAZ_00027337 -->

    <owl:NamedIndividual rdf:about="http://purl.obolibrary.org/obo/GAZ_00027337">
        <rdf:type rdf:resource="http://purl.obolibrary.org/obo/ENVO_00000004"/>
        <obo:RO_0001025 rdf:resource="http://purl.obolibrary.org/obo/GAZ_00014869"/>
        <obo:IAO_0000115>A sum (district) of Tov Province in Mongolia.</obo:IAO_0000115>
        <oboInOwl:hasOBONamespace>GAZ</oboInOwl:hasOBONamespace>
        <oboInOwl:id>GAZ:00027337</oboInOwl:id>
        <rdfs:label>Bayantsagaan District</rdfs:label>
    </owl:NamedIndividual>
    


    <!-- http://purl.obolibrary.org/obo/GAZ_00027338 -->

    <owl:NamedIndividual rdf:about="http://purl.obolibrary.org/obo/GAZ_00027338">
        <rdf:type rdf:resource="http://purl.obolibrary.org/obo/ENVO_00000004"/>
        <obo:RO_0001025 rdf:resource="http://purl.obolibrary.org/obo/GAZ_00014869"/>
        <obo:IAO_0000115>A sum (district) of Tov Province in Mongolia.</obo:IAO_0000115>
        <oboInOwl:hasOBONamespace>GAZ</oboInOwl:hasOBONamespace>
        <oboInOwl:id>GAZ:00027338</oboInOwl:id>
        <rdfs:label>Mongonmorit District</rdfs:label>
    </owl:NamedIndividual>
    


    <!-- http://purl.obolibrary.org/obo/GAZ_00027339 -->

    <owl:NamedIndividual rdf:about="http://purl.obolibrary.org/obo/GAZ_00027339">
        <rdf:type rdf:resource="http://purl.obolibrary.org/obo/ENVO_00000004"/>
        <obo:RO_0001025 rdf:resource="http://purl.obolibrary.org/obo/GAZ_00014869"/>
        <obo:IAO_0000115>A sum (district) of Tov Province in Mongolia.</obo:IAO_0000115>
        <oboInOwl:hasOBONamespace>GAZ</oboInOwl:hasOBONamespace>
        <oboInOwl:id>GAZ:00027339</oboInOwl:id>
        <rdfs:label>Erdene District</rdfs:label>
    </owl:NamedIndividual>
    


    <!-- http://purl.obolibrary.org/obo/GAZ_00027340 -->

    <owl:NamedIndividual rdf:about="http://purl.obolibrary.org/obo/GAZ_00027340">
        <rdf:type rdf:resource="http://purl.obolibrary.org/obo/ENVO_00000004"/>
        <obo:RO_0001025 rdf:resource="http://purl.obolibrary.org/obo/GAZ_00014869"/>
        <obo:IAO_0000115>A sum (district) of Tov Province in Mongolia.</obo:IAO_0000115>
        <oboInOwl:hasOBONamespace>GAZ</oboInOwl:hasOBONamespace>
        <oboInOwl:id>GAZ:00027340</oboInOwl:id>
        <rdfs:label>Erdenesant District</rdfs:label>
    </owl:NamedIndividual>
    


    <!-- http://purl.obolibrary.org/obo/GAZ_00027341 -->

    <owl:NamedIndividual rdf:about="http://purl.obolibrary.org/obo/GAZ_00027341">
        <rdf:type rdf:resource="http://purl.obolibrary.org/obo/ENVO_00000004"/>
        <obo:RO_0001025 rdf:resource="http://purl.obolibrary.org/obo/GAZ_00014869"/>
        <obo:IAO_0000115>A sum (district) of Tov Province in Mongolia.</obo:IAO_0000115>
        <oboInOwl:hasOBONamespace>GAZ</oboInOwl:hasOBONamespace>
        <oboInOwl:id>GAZ:00027341</oboInOwl:id>
        <rdfs:label>Sumber District</rdfs:label>
    </owl:NamedIndividual>
    


    <!-- http://purl.obolibrary.org/obo/GAZ_00027342 -->

    <owl:NamedIndividual rdf:about="http://purl.obolibrary.org/obo/GAZ_00027342">
        <rdf:type rdf:resource="http://purl.obolibrary.org/obo/ENVO_00000004"/>
        <obo:RO_0001025 rdf:resource="http://purl.obolibrary.org/obo/GAZ_00014869"/>
        <obo:IAO_0000115>A sum (district) of Tov Province in Mongolia.</obo:IAO_0000115>
        <oboInOwl:hasOBONamespace>GAZ</oboInOwl:hasOBONamespace>
        <oboInOwl:id>GAZ:00027342</oboInOwl:id>
        <rdfs:label>Ugtaal District</rdfs:label>
    </owl:NamedIndividual>
    


    <!-- http://purl.obolibrary.org/obo/GAZ_00027343 -->

    <owl:NamedIndividual rdf:about="http://purl.obolibrary.org/obo/GAZ_00027343">
        <rdf:type rdf:resource="http://purl.obolibrary.org/obo/ENVO_00000004"/>
        <obo:RO_0001025 rdf:resource="http://purl.obolibrary.org/obo/GAZ_00014869"/>
        <obo:IAO_0000115>A sum (district) of Tov Province in Mongolia.</obo:IAO_0000115>
        <oboInOwl:hasOBONamespace>GAZ</oboInOwl:hasOBONamespace>
        <oboInOwl:id>GAZ:00027343</oboInOwl:id>
        <rdfs:label>Altanbulag District</rdfs:label>
    </owl:NamedIndividual>
    


    <!-- http://purl.obolibrary.org/obo/GAZ_00027344 -->

    <owl:NamedIndividual rdf:about="http://purl.obolibrary.org/obo/GAZ_00027344">
        <rdf:type rdf:resource="http://purl.obolibrary.org/obo/ENVO_00000004"/>
        <obo:RO_0001025 rdf:resource="http://purl.obolibrary.org/obo/GAZ_00014869"/>
        <obo:IAO_0000115>A sum (district) of Tov Province in Mongolia.</obo:IAO_0000115>
        <oboInOwl:hasOBONamespace>GAZ</oboInOwl:hasOBONamespace>
        <oboInOwl:id>GAZ:00027344</oboInOwl:id>
        <rdfs:label>Lun District</rdfs:label>
    </owl:NamedIndividual>
    


    <!-- http://purl.obolibrary.org/obo/GAZ_00027345 -->

    <owl:NamedIndividual rdf:about="http://purl.obolibrary.org/obo/GAZ_00027345">
        <rdf:type rdf:resource="http://purl.obolibrary.org/obo/ENVO_00000004"/>
        <obo:RO_0001025 rdf:resource="http://purl.obolibrary.org/obo/GAZ_00014869"/>
        <obo:IAO_0000115>A sum (district) of Tov Province in Mongolia.</obo:IAO_0000115>
        <oboInOwl:hasOBONamespace>GAZ</oboInOwl:hasOBONamespace>
        <oboInOwl:id>GAZ:00027345</oboInOwl:id>
        <rdfs:label>Delgerkhaan District</rdfs:label>
    </owl:NamedIndividual>
    


    <!-- http://purl.obolibrary.org/obo/GAZ_00027346 -->

    <owl:NamedIndividual rdf:about="http://purl.obolibrary.org/obo/GAZ_00027346">
        <rdf:type rdf:resource="http://purl.obolibrary.org/obo/ENVO_00000004"/>
        <obo:RO_0001025 rdf:resource="http://purl.obolibrary.org/obo/GAZ_00014869"/>
        <obo:IAO_0000115>A sum (district) of Tov Province in Mongolia.</obo:IAO_0000115>
        <oboInOwl:hasOBONamespace>GAZ</oboInOwl:hasOBONamespace>
        <oboInOwl:id>GAZ:00027346</oboInOwl:id>
        <rdfs:label>Zaamar District</rdfs:label>
    </owl:NamedIndividual>
    


    <!-- http://purl.obolibrary.org/obo/GAZ_00027347 -->

    <owl:NamedIndividual rdf:about="http://purl.obolibrary.org/obo/GAZ_00027347">
        <rdf:type rdf:resource="http://purl.obolibrary.org/obo/ENVO_00000004"/>
        <obo:RO_0001025 rdf:resource="http://purl.obolibrary.org/obo/GAZ_00014869"/>
        <obo:IAO_0000115>A sum (district) of Tov Province in Mongolia.</obo:IAO_0000115>
        <oboInOwl:hasOBONamespace>GAZ</oboInOwl:hasOBONamespace>
        <oboInOwl:id>GAZ:00027347</oboInOwl:id>
        <rdfs:label>Sergelen District</rdfs:label>
    </owl:NamedIndividual>
    


    <!-- http://purl.obolibrary.org/obo/GAZ_00027348 -->

    <owl:NamedIndividual rdf:about="http://purl.obolibrary.org/obo/GAZ_00027348">
        <rdf:type rdf:resource="http://purl.obolibrary.org/obo/ENVO_00000004"/>
        <obo:RO_0001025 rdf:resource="http://purl.obolibrary.org/obo/GAZ_00014869"/>
        <obo:IAO_0000115>A sum (district) of Tov Province in Mongolia.</obo:IAO_0000115>
        <oboInOwl:hasOBONamespace>GAZ</oboInOwl:hasOBONamespace>
        <oboInOwl:id>GAZ:00027348</oboInOwl:id>
        <rdfs:label>Tseel District</rdfs:label>
    </owl:NamedIndividual>
    


    <!-- http://purl.obolibrary.org/obo/GAZ_00027349 -->

    <owl:NamedIndividual rdf:about="http://purl.obolibrary.org/obo/GAZ_00027349">
        <rdf:type rdf:resource="http://purl.obolibrary.org/obo/ENVO_00000004"/>
        <obo:RO_0001025 rdf:resource="http://purl.obolibrary.org/obo/GAZ_00014869"/>
        <obo:IAO_0000115>A sum (district) of Tov Province in Mongolia.</obo:IAO_0000115>
        <oboInOwl:hasOBONamespace>GAZ</oboInOwl:hasOBONamespace>
        <oboInOwl:id>GAZ:00027349</oboInOwl:id>
        <rdfs:label>Argalant District</rdfs:label>
    </owl:NamedIndividual>
    


    <!-- http://purl.obolibrary.org/obo/GAZ_00027350 -->

    <owl:NamedIndividual rdf:about="http://purl.obolibrary.org/obo/GAZ_00027350">
        <rdf:type rdf:resource="http://purl.obolibrary.org/obo/ENVO_00000004"/>
        <obo:RO_0001025 rdf:resource="http://purl.obolibrary.org/obo/GAZ_00014869"/>
        <obo:IAO_0000115>A sum (district) of Tov Province in Mongolia.</obo:IAO_0000115>
        <oboInOwl:hasOBONamespace>GAZ</oboInOwl:hasOBONamespace>
        <oboInOwl:id>GAZ:00027350</oboInOwl:id>
        <rdfs:label>Jargalant District</rdfs:label>
    </owl:NamedIndividual>
    


    <!-- http://purl.obolibrary.org/obo/GAZ_00027351 -->

    <owl:NamedIndividual rdf:about="http://purl.obolibrary.org/obo/GAZ_00027351">
        <rdf:type rdf:resource="http://purl.obolibrary.org/obo/ENVO_00000004"/>
        <obo:RO_0001025 rdf:resource="http://purl.obolibrary.org/obo/GAZ_00014869"/>
        <obo:IAO_0000115>A sum (district) of Tov Province in Mongolia.</obo:IAO_0000115>
        <oboInOwl:hasOBONamespace>GAZ</oboInOwl:hasOBONamespace>
        <oboInOwl:id>GAZ:00027351</oboInOwl:id>
        <rdfs:label>Buren District</rdfs:label>
    </owl:NamedIndividual>
    


    <!-- http://purl.obolibrary.org/obo/GAZ_00027352 -->

    <owl:NamedIndividual rdf:about="http://purl.obolibrary.org/obo/GAZ_00027352">
        <rdf:type rdf:resource="http://purl.obolibrary.org/obo/ENVO_00000004"/>
        <obo:RO_0001025 rdf:resource="http://purl.obolibrary.org/obo/GAZ_00014869"/>
        <obo:IAO_0000115>A sum (district) of Tov Province in Mongolia.</obo:IAO_0000115>
        <oboInOwl:hasOBONamespace>GAZ</oboInOwl:hasOBONamespace>
        <oboInOwl:id>GAZ:00027352</oboInOwl:id>
        <rdfs:label>Ondorshireet District</rdfs:label>
    </owl:NamedIndividual>
    


    <!-- http://purl.obolibrary.org/obo/GAZ_00027353 -->

    <owl:NamedIndividual rdf:about="http://purl.obolibrary.org/obo/GAZ_00027353">
        <rdf:type rdf:resource="http://purl.obolibrary.org/obo/ENVO_00000004"/>
        <obo:RO_0001025 rdf:resource="http://purl.obolibrary.org/obo/GAZ_00014876"/>
        <obo:IAO_0000115>A sum (district) of Uvs Province in Mongolia.</obo:IAO_0000115>
        <oboInOwl:hasOBONamespace>GAZ</oboInOwl:hasOBONamespace>
        <oboInOwl:id>GAZ:00027353</oboInOwl:id>
        <rdfs:label>Baruunturuun District</rdfs:label>
    </owl:NamedIndividual>
    


    <!-- http://purl.obolibrary.org/obo/GAZ_00027354 -->

    <owl:NamedIndividual rdf:about="http://purl.obolibrary.org/obo/GAZ_00027354">
        <rdf:type rdf:resource="http://purl.obolibrary.org/obo/ENVO_00000004"/>
        <obo:RO_0001025 rdf:resource="http://purl.obolibrary.org/obo/GAZ_00014869"/>
        <obo:IAO_0000115>A sum (district) of Tov Province in Mongolia. The sum was founded in 1923, under the name Gun sum and as part of the Tusheet Khan aimag&apos;s Darkhan chin wangyn khoshuu. 1924 it was renamed to Batdelger uulyn sum, and in 1931 it was renamed again. In 1956 it was split between the Bayan and Erdene sums, with most of the territory going to the latter. In 1959, the Bayandelger sum was re-established.</obo:IAO_0000115>
        <oboInOwl:hasOBONamespace>GAZ</oboInOwl:hasOBONamespace>
        <oboInOwl:id>GAZ:00027354</oboInOwl:id>
        <rdfs:label>Bayandelger District</rdfs:label>
    </owl:NamedIndividual>
    


    <!-- http://purl.obolibrary.org/obo/GAZ_00027355 -->

    <owl:NamedIndividual rdf:about="http://purl.obolibrary.org/obo/GAZ_00027355">
        <rdf:type rdf:resource="http://purl.obolibrary.org/obo/ENVO_00000004"/>
        <obo:RO_0001025 rdf:resource="http://purl.obolibrary.org/obo/GAZ_00014876"/>
        <obo:IAO_0000115>A sum (district) of Uvs Province in Mongolia.</obo:IAO_0000115>
        <oboInOwl:hasOBONamespace>GAZ</oboInOwl:hasOBONamespace>
        <oboInOwl:id>GAZ:00027355</oboInOwl:id>
        <rdfs:label>Naranbulag District</rdfs:label>
    </owl:NamedIndividual>
    


    <!-- http://purl.obolibrary.org/obo/GAZ_00027356 -->

    <owl:NamedIndividual rdf:about="http://purl.obolibrary.org/obo/GAZ_00027356">
        <rdf:type rdf:resource="http://purl.obolibrary.org/obo/ENVO_00000004"/>
        <obo:RO_0001025 rdf:resource="http://purl.obolibrary.org/obo/GAZ_00014869"/>
        <obo:IAO_0000115>A sum (district) of Tov Province in Mongolia.</obo:IAO_0000115>
        <oboInOwl:hasOBONamespace>GAZ</oboInOwl:hasOBONamespace>
        <oboInOwl:id>GAZ:00027356</oboInOwl:id>
        <rdfs:label>Bayankhangai District</rdfs:label>
    </owl:NamedIndividual>
    


    <!-- http://purl.obolibrary.org/obo/GAZ_00027357 -->

    <owl:NamedIndividual rdf:about="http://purl.obolibrary.org/obo/GAZ_00027357">
        <rdf:type rdf:resource="http://purl.obolibrary.org/obo/ENVO_00000004"/>
        <obo:RO_0001025 rdf:resource="http://purl.obolibrary.org/obo/GAZ_00014869"/>
        <obo:IAO_0000115>A sum (district) of Tov Province in Mongolia.</obo:IAO_0000115>
        <oboInOwl:hasOBONamespace>GAZ</oboInOwl:hasOBONamespace>
        <oboInOwl:id>GAZ:00027357</oboInOwl:id>
        <rdfs:label>Arkhust District</rdfs:label>
    </owl:NamedIndividual>
    


    <!-- http://purl.obolibrary.org/obo/GAZ_00027358 -->

    <owl:NamedIndividual rdf:about="http://purl.obolibrary.org/obo/GAZ_00027358">
        <rdf:type rdf:resource="http://purl.obolibrary.org/obo/ENVO_00000004"/>
        <obo:RO_0001025 rdf:resource="http://purl.obolibrary.org/obo/GAZ_00014869"/>
        <obo:IAO_0000115>A sum (district) of Tov Province in Mongolia.</obo:IAO_0000115>
        <oboInOwl:hasOBONamespace>GAZ</oboInOwl:hasOBONamespace>
        <oboInOwl:id>GAZ:00027358</oboInOwl:id>
        <rdfs:label>Bayanjargalan District</rdfs:label>
    </owl:NamedIndividual>
    


    <!-- http://purl.obolibrary.org/obo/GAZ_00027359 -->

    <owl:NamedIndividual rdf:about="http://purl.obolibrary.org/obo/GAZ_00027359">
        <rdf:type rdf:resource="http://purl.obolibrary.org/obo/ENVO_00000004"/>
        <obo:RO_0001025 rdf:resource="http://purl.obolibrary.org/obo/GAZ_00014869"/>
        <obo:IAO_0000115>A sum (district) of Tov Province in Mongolia.</obo:IAO_0000115>
        <oboInOwl:hasOBONamespace>GAZ</oboInOwl:hasOBONamespace>
        <oboInOwl:id>GAZ:00027359</oboInOwl:id>
        <rdfs:label>Bayan-Onjuul District</rdfs:label>
    </owl:NamedIndividual>
    


    <!-- http://purl.obolibrary.org/obo/GAZ_00027360 -->

    <owl:NamedIndividual rdf:about="http://purl.obolibrary.org/obo/GAZ_00027360">
        <rdf:type rdf:resource="http://purl.obolibrary.org/obo/ENVO_00000004"/>
        <obo:RO_0001025 rdf:resource="http://purl.obolibrary.org/obo/GAZ_00014876"/>
        <obo:IAO_0000115>A sum (district) of Uvs Province in Mongolia.</obo:IAO_0000115>
        <oboInOwl:hasOBONamespace>GAZ</oboInOwl:hasOBONamespace>
        <oboInOwl:id>GAZ:00027360</oboInOwl:id>
        <rdfs:label>Turgen District</rdfs:label>
    </owl:NamedIndividual>
    


    <!-- http://purl.obolibrary.org/obo/GAZ_00027361 -->

    <owl:NamedIndividual rdf:about="http://purl.obolibrary.org/obo/GAZ_00027361">
        <rdf:type rdf:resource="http://purl.obolibrary.org/obo/ENVO_00000004"/>
        <obo:RO_0001025 rdf:resource="http://purl.obolibrary.org/obo/GAZ_00014876"/>
        <obo:IAO_0000115>A sum (district) of Uvs Province in Mongolia.</obo:IAO_0000115>
        <oboInOwl:hasOBONamespace>GAZ</oboInOwl:hasOBONamespace>
        <oboInOwl:id>GAZ:00027361</oboInOwl:id>
        <rdfs:label>Olgii District</rdfs:label>
    </owl:NamedIndividual>
    


    <!-- http://purl.obolibrary.org/obo/GAZ_00027362 -->

    <owl:NamedIndividual rdf:about="http://purl.obolibrary.org/obo/GAZ_00027362">
        <rdf:type rdf:resource="http://purl.obolibrary.org/obo/ENVO_00000004"/>
        <obo:RO_0001025 rdf:resource="http://purl.obolibrary.org/obo/GAZ_00014876"/>
        <obo:IAO_0000115>A sum (district) of Uvs Province in Mongolia. It lies on the southern shore of Uvs Nuur.</obo:IAO_0000115>
        <oboInOwl:hasOBONamespace>GAZ</oboInOwl:hasOBONamespace>
        <oboInOwl:id>GAZ:00027362</oboInOwl:id>
        <rdfs:label>Zuungovi District</rdfs:label>
    </owl:NamedIndividual>
    


    <!-- http://purl.obolibrary.org/obo/GAZ_00027363 -->

    <owl:NamedIndividual rdf:about="http://purl.obolibrary.org/obo/GAZ_00027363">
        <rdf:type rdf:resource="http://purl.obolibrary.org/obo/ENVO_00000004"/>
        <obo:RO_0001025 rdf:resource="http://purl.obolibrary.org/obo/GAZ_00014876"/>
        <obo:IAO_0000115>A sum (district) of Uvs Province in Mongolia.</obo:IAO_0000115>
        <oboInOwl:hasOBONamespace>GAZ</oboInOwl:hasOBONamespace>
        <oboInOwl:id>GAZ:00027363</oboInOwl:id>
        <rdfs:label>Sagil District</rdfs:label>
    </owl:NamedIndividual>
    


    <!-- http://purl.obolibrary.org/obo/GAZ_00027364 -->

    <owl:NamedIndividual rdf:about="http://purl.obolibrary.org/obo/GAZ_00027364">
        <rdf:type rdf:resource="http://purl.obolibrary.org/obo/ENVO_00000004"/>
        <obo:RO_0001025 rdf:resource="http://purl.obolibrary.org/obo/GAZ_00014876"/>
        <obo:IAO_0000115>A sum (district) of Uvs Province in Mongolia.</obo:IAO_0000115>
        <oboInOwl:hasOBONamespace>GAZ</oboInOwl:hasOBONamespace>
        <oboInOwl:id>GAZ:00027364</oboInOwl:id>
        <rdfs:label>Ondorkhangai District</rdfs:label>
    </owl:NamedIndividual>
    


    <!-- http://purl.obolibrary.org/obo/GAZ_00027365 -->

    <owl:NamedIndividual rdf:about="http://purl.obolibrary.org/obo/GAZ_00027365">
        <rdf:type rdf:resource="http://purl.obolibrary.org/obo/ENVO_00000004"/>
        <obo:RO_0001025 rdf:resource="http://purl.obolibrary.org/obo/GAZ_00014876"/>
        <obo:IAO_0000115>A sum (district) of Uvs Province in Mongolia.</obo:IAO_0000115>
        <oboInOwl:hasOBONamespace>GAZ</oboInOwl:hasOBONamespace>
        <oboInOwl:id>GAZ:00027365</oboInOwl:id>
        <rdfs:label>Zavkhan District</rdfs:label>
    </owl:NamedIndividual>
    


    <!-- http://purl.obolibrary.org/obo/GAZ_00027366 -->

    <owl:NamedIndividual rdf:about="http://purl.obolibrary.org/obo/GAZ_00027366">
        <rdf:type rdf:resource="http://purl.obolibrary.org/obo/ENVO_00000004"/>
        <obo:RO_0001025 rdf:resource="http://purl.obolibrary.org/obo/GAZ_00014876"/>
        <obo:IAO_0000115>A sum (district) of Uvs Province in Mongolia.</obo:IAO_0000115>
        <oboInOwl:hasOBONamespace>GAZ</oboInOwl:hasOBONamespace>
        <oboInOwl:id>GAZ:00027366</oboInOwl:id>
        <rdfs:label>Omnogovi District</rdfs:label>
    </owl:NamedIndividual>
    


    <!-- http://purl.obolibrary.org/obo/GAZ_00027367 -->

    <owl:NamedIndividual rdf:about="http://purl.obolibrary.org/obo/GAZ_00027367">
        <rdf:type rdf:resource="http://purl.obolibrary.org/obo/ENVO_00000004"/>
        <obo:RO_0001025 rdf:resource="http://purl.obolibrary.org/obo/GAZ_00014876"/>
        <obo:IAO_0000115>A sum (district) of Uvs Province in Mongolia.</obo:IAO_0000115>
        <oboInOwl:hasOBONamespace>GAZ</oboInOwl:hasOBONamespace>
        <oboInOwl:id>GAZ:00027367</oboInOwl:id>
        <rdfs:label>Zuunkhangai District</rdfs:label>
    </owl:NamedIndividual>
    


    <!-- http://purl.obolibrary.org/obo/GAZ_00027368 -->

    <owl:NamedIndividual rdf:about="http://purl.obolibrary.org/obo/GAZ_00027368">
        <rdf:type rdf:resource="http://purl.obolibrary.org/obo/ENVO_00000004"/>
        <obo:RO_0001025 rdf:resource="http://purl.obolibrary.org/obo/GAZ_00014876"/>
        <obo:IAO_0000115>A sum (district) of Uvs Province in Mongolia.</obo:IAO_0000115>
        <oboInOwl:hasOBONamespace>GAZ</oboInOwl:hasOBONamespace>
        <oboInOwl:id>GAZ:00027368</oboInOwl:id>
        <rdfs:label>Tsagaanhairhan District</rdfs:label>
    </owl:NamedIndividual>
    


    <!-- http://purl.obolibrary.org/obo/GAZ_00027369 -->

    <owl:NamedIndividual rdf:about="http://purl.obolibrary.org/obo/GAZ_00027369">
        <rdf:type rdf:resource="http://purl.obolibrary.org/obo/ENVO_00000004"/>
        <obo:RO_0001025 rdf:resource="http://purl.obolibrary.org/obo/GAZ_00014876"/>
        <obo:IAO_0000115>A sum (district) of Uvs Province in Mongolia.</obo:IAO_0000115>
        <oboInOwl:hasOBONamespace>GAZ</oboInOwl:hasOBONamespace>
        <oboInOwl:id>GAZ:00027369</oboInOwl:id>
        <rdfs:label>Tarialan District</rdfs:label>
    </owl:NamedIndividual>
    


    <!-- http://purl.obolibrary.org/obo/GAZ_00027370 -->

    <owl:NamedIndividual rdf:about="http://purl.obolibrary.org/obo/GAZ_00027370">
        <rdf:type rdf:resource="http://purl.obolibrary.org/obo/ENVO_00000004"/>
        <obo:RO_0001025 rdf:resource="http://purl.obolibrary.org/obo/GAZ_00014876"/>
        <obo:IAO_0000115>A sum (district) of Uvs Province in Mongolia.</obo:IAO_0000115>
        <oboInOwl:hasOBONamespace>GAZ</oboInOwl:hasOBONamespace>
        <oboInOwl:id>GAZ:00027370</oboInOwl:id>
        <rdfs:label>Tes District</rdfs:label>
    </owl:NamedIndividual>
    


    <!-- http://purl.obolibrary.org/obo/GAZ_00027371 -->

    <owl:NamedIndividual rdf:about="http://purl.obolibrary.org/obo/GAZ_00027371">
        <rdf:type rdf:resource="http://purl.obolibrary.org/obo/ENVO_00000004"/>
        <obo:RO_0001025 rdf:resource="http://purl.obolibrary.org/obo/GAZ_00014876"/>
        <obo:IAO_0000115>A sum (district) of Uvs Province in Mongolia. The capital of Uvs Province in Mongolia. It is located near the southwestern shore of the lake Uvs Nuur and on the slopes of the Kharkhiraa mountains, close to the Russian border.</obo:IAO_0000115>
        <oboInOwl:hasOBONamespace>GAZ</oboInOwl:hasOBONamespace>
        <oboInOwl:id>GAZ:00027371</oboInOwl:id>
        <rdfs:label>Ulaangom District</rdfs:label>
    </owl:NamedIndividual>
    


    <!-- http://purl.obolibrary.org/obo/GAZ_00027372 -->

    <owl:NamedIndividual rdf:about="http://purl.obolibrary.org/obo/GAZ_00027372">
        <rdf:type rdf:resource="http://purl.obolibrary.org/obo/ENVO_00000004"/>
        <obo:RO_0001025 rdf:resource="http://purl.obolibrary.org/obo/GAZ_00014877"/>
        <obo:IAO_0000115>A sum (district) of Zavkhan Province in western Mongolia.</obo:IAO_0000115>
        <oboInOwl:hasOBONamespace>GAZ</oboInOwl:hasOBONamespace>
        <oboInOwl:id>GAZ:00027372</oboInOwl:id>
        <rdfs:label>Tsagaankhairkhan District</rdfs:label>
    </owl:NamedIndividual>
    


    <!-- http://purl.obolibrary.org/obo/GAZ_00027373 -->

    <owl:NamedIndividual rdf:about="http://purl.obolibrary.org/obo/GAZ_00027373">
        <rdf:type rdf:resource="http://purl.obolibrary.org/obo/ENVO_00000004"/>
        <obo:RO_0001025 rdf:resource="http://purl.obolibrary.org/obo/GAZ_00014877"/>
        <obo:IAO_0000115>A sum (district) of Zavkhan Province in western Mongolia.</obo:IAO_0000115>
        <oboInOwl:hasOBONamespace>GAZ</oboInOwl:hasOBONamespace>
        <oboInOwl:id>GAZ:00027373</oboInOwl:id>
        <rdfs:label>Tudevtei District</rdfs:label>
    </owl:NamedIndividual>
    


    <!-- http://purl.obolibrary.org/obo/GAZ_00027374 -->

    <owl:NamedIndividual rdf:about="http://purl.obolibrary.org/obo/GAZ_00027374">
        <rdf:type rdf:resource="http://purl.obolibrary.org/obo/ENVO_00000004"/>
        <obo:RO_0001025 rdf:resource="http://purl.obolibrary.org/obo/GAZ_00014877"/>
        <obo:IAO_0000115>A sum (district) of Zavkhan Province in western Mongolia.</obo:IAO_0000115>
        <oboInOwl:hasOBONamespace>GAZ</oboInOwl:hasOBONamespace>
        <oboInOwl:id>GAZ:00027374</oboInOwl:id>
        <rdfs:label>Aldarkhaan District</rdfs:label>
    </owl:NamedIndividual>
    


    <!-- http://purl.obolibrary.org/obo/GAZ_00027375 -->

    <owl:NamedIndividual rdf:about="http://purl.obolibrary.org/obo/GAZ_00027375">
        <rdf:type rdf:resource="http://purl.obolibrary.org/obo/ENVO_00000004"/>
        <obo:RO_0001025 rdf:resource="http://purl.obolibrary.org/obo/GAZ_00014877"/>
        <obo:IAO_0000115>A sum (district) of Zavkhan Province in western Mongolia.</obo:IAO_0000115>
        <oboInOwl:hasOBONamespace>GAZ</oboInOwl:hasOBONamespace>
        <oboInOwl:id>GAZ:00027375</oboInOwl:id>
        <rdfs:label>Urgamal District</rdfs:label>
    </owl:NamedIndividual>
    


    <!-- http://purl.obolibrary.org/obo/GAZ_00027376 -->

    <owl:NamedIndividual rdf:about="http://purl.obolibrary.org/obo/GAZ_00027376">
        <obo:RO_0001025 rdf:resource="http://purl.obolibrary.org/obo/GAZ_00014877"/>
        <obo:IAO_0000115>A populated place. A city in Mongolia. It is located in the western part of the country, 1,115 km from the capital Ulan Bator. Uliastai is the capital of Zavkhan Province.</obo:IAO_0000115>
        <oboInOwl:hasOBONamespace>GAZ</oboInOwl:hasOBONamespace>
        <oboInOwl:id>GAZ:00027376</oboInOwl:id>
        <rdfs:label>Uliastai City</rdfs:label>
    </owl:NamedIndividual>
    


    <!-- http://purl.obolibrary.org/obo/GAZ_00027377 -->

    <owl:NamedIndividual rdf:about="http://purl.obolibrary.org/obo/GAZ_00027377">
        <rdf:type rdf:resource="http://purl.obolibrary.org/obo/ENVO_00000004"/>
        <obo:RO_0001025 rdf:resource="http://purl.obolibrary.org/obo/GAZ_00014877"/>
        <obo:IAO_0000115>A sum (district) of Zavkhan Province in western Mongolia.</obo:IAO_0000115>
        <oboInOwl:hasOBONamespace>GAZ</oboInOwl:hasOBONamespace>
        <oboInOwl:id>GAZ:00027377</oboInOwl:id>
        <rdfs:label>Tsagaanchuluut District</rdfs:label>
    </owl:NamedIndividual>
    


    <!-- http://purl.obolibrary.org/obo/GAZ_00027378 -->

    <owl:NamedIndividual rdf:about="http://purl.obolibrary.org/obo/GAZ_00027378">
        <rdf:type rdf:resource="http://purl.obolibrary.org/obo/ENVO_00000004"/>
        <obo:RO_0001025 rdf:resource="http://purl.obolibrary.org/obo/GAZ_00014877"/>
        <obo:IAO_0000115>A sum (district) of Zavkhan Province in western Mongolia.</obo:IAO_0000115>
        <oboInOwl:hasOBONamespace>GAZ</oboInOwl:hasOBONamespace>
        <oboInOwl:id>GAZ:00027378</oboInOwl:id>
        <rdfs:label>Ikh-Uul District</rdfs:label>
    </owl:NamedIndividual>
    


    <!-- http://purl.obolibrary.org/obo/GAZ_00027379 -->

    <owl:NamedIndividual rdf:about="http://purl.obolibrary.org/obo/GAZ_00027379">
        <rdf:type rdf:resource="http://purl.obolibrary.org/obo/ENVO_00000004"/>
        <obo:RO_0001025 rdf:resource="http://purl.obolibrary.org/obo/GAZ_00014877"/>
        <obo:IAO_0000115>A sum (district) of Zavkhan Province in western Mongolia.</obo:IAO_0000115>
        <oboInOwl:hasOBONamespace>GAZ</oboInOwl:hasOBONamespace>
        <oboInOwl:id>GAZ:00027379</oboInOwl:id>
        <rdfs:label>Shiluustei District</rdfs:label>
    </owl:NamedIndividual>
    


    <!-- http://purl.obolibrary.org/obo/GAZ_00027380 -->

    <owl:NamedIndividual rdf:about="http://purl.obolibrary.org/obo/GAZ_00027380">
        <rdf:type rdf:resource="http://purl.obolibrary.org/obo/ENVO_00000004"/>
        <obo:RO_0001025 rdf:resource="http://purl.obolibrary.org/obo/GAZ_00014877"/>
        <obo:IAO_0000115>A sum (district) of Zavkhan Province in western Mongolia.</obo:IAO_0000115>
        <oboInOwl:hasOBONamespace>GAZ</oboInOwl:hasOBONamespace>
        <oboInOwl:id>GAZ:00027380</oboInOwl:id>
        <rdfs:label>Tes District</rdfs:label>
    </owl:NamedIndividual>
    


    <!-- http://purl.obolibrary.org/obo/GAZ_00027381 -->

    <owl:NamedIndividual rdf:about="http://purl.obolibrary.org/obo/GAZ_00027381">
        <rdf:type rdf:resource="http://purl.obolibrary.org/obo/ENVO_00000004"/>
        <obo:RO_0001025 rdf:resource="http://purl.obolibrary.org/obo/GAZ_00014877"/>
        <obo:IAO_0000115>A sum (district) of Zavkhan Province in western Mongolia.</obo:IAO_0000115>
        <oboInOwl:hasOBONamespace>GAZ</oboInOwl:hasOBONamespace>
        <oboInOwl:id>GAZ:00027381</oboInOwl:id>
        <rdfs:label>Ider District</rdfs:label>
    </owl:NamedIndividual>
    


    <!-- http://purl.obolibrary.org/obo/GAZ_00027382 -->

    <owl:NamedIndividual rdf:about="http://purl.obolibrary.org/obo/GAZ_00027382">
        <rdf:type rdf:resource="http://purl.obolibrary.org/obo/ENVO_00000004"/>
        <obo:RO_0001025 rdf:resource="http://purl.obolibrary.org/obo/GAZ_00014877"/>
        <obo:IAO_0000115>A sum (district) of Zavkhan Province in western Mongolia.</obo:IAO_0000115>
        <oboInOwl:hasOBONamespace>GAZ</oboInOwl:hasOBONamespace>
        <oboInOwl:id>GAZ:00027382</oboInOwl:id>
        <rdfs:label>Asgat District</rdfs:label>
    </owl:NamedIndividual>
    


    <!-- http://purl.obolibrary.org/obo/GAZ_00027383 -->

    <owl:NamedIndividual rdf:about="http://purl.obolibrary.org/obo/GAZ_00027383">
        <obo:RO_0001025 rdf:resource="http://purl.obolibrary.org/obo/GAZ_00014877"/>
        <oboInOwl:hasOBONamespace>GAZ</oboInOwl:hasOBONamespace>
        <oboInOwl:id>GAZ:00027383</oboInOwl:id>
        <rdfs:label>Otgon District</rdfs:label>
    </owl:NamedIndividual>
    


    <!-- http://purl.obolibrary.org/obo/GAZ_00027384 -->

    <owl:NamedIndividual rdf:about="http://purl.obolibrary.org/obo/GAZ_00027384">
        <rdf:type rdf:resource="http://purl.obolibrary.org/obo/ENVO_00000004"/>
        <obo:RO_0001025 rdf:resource="http://purl.obolibrary.org/obo/GAZ_00014877"/>
        <obo:IAO_0000115>A sum (district) of Zavkhan Province in western Mongolia.</obo:IAO_0000115>
        <oboInOwl:hasOBONamespace>GAZ</oboInOwl:hasOBONamespace>
        <oboInOwl:id>GAZ:00027384</oboInOwl:id>
        <rdfs:label>Dorvoljin District</rdfs:label>
    </owl:NamedIndividual>
    


    <!-- http://purl.obolibrary.org/obo/GAZ_00027385 -->

    <owl:NamedIndividual rdf:about="http://purl.obolibrary.org/obo/GAZ_00027385">
        <rdf:type rdf:resource="http://purl.obolibrary.org/obo/ENVO_00000004"/>
        <obo:RO_0001025 rdf:resource="http://purl.obolibrary.org/obo/GAZ_00014877"/>
        <obo:IAO_0000115>A sum (district) of Zavkhan Province in western Mongolia.</obo:IAO_0000115>
        <oboInOwl:hasOBONamespace>GAZ</oboInOwl:hasOBONamespace>
        <oboInOwl:id>GAZ:00027385</oboInOwl:id>
        <rdfs:label>Zavkhanmandal District</rdfs:label>
    </owl:NamedIndividual>
    


    <!-- http://purl.obolibrary.org/obo/GAZ_00027386 -->

    <owl:NamedIndividual rdf:about="http://purl.obolibrary.org/obo/GAZ_00027386">
        <rdf:type rdf:resource="http://purl.obolibrary.org/obo/ENVO_00000004"/>
        <obo:RO_0001025 rdf:resource="http://purl.obolibrary.org/obo/GAZ_00014877"/>
        <obo:IAO_0000115>A sum (district) of Zavkhan Province in western Mongolia.</obo:IAO_0000115>
        <oboInOwl:hasOBONamespace>GAZ</oboInOwl:hasOBONamespace>
        <oboInOwl:id>GAZ:00027386</oboInOwl:id>
        <rdfs:label>Yaruu District</rdfs:label>
    </owl:NamedIndividual>
    


    <!-- http://purl.obolibrary.org/obo/GAZ_00027387 -->

    <owl:NamedIndividual rdf:about="http://purl.obolibrary.org/obo/GAZ_00027387">
        <rdf:type rdf:resource="http://purl.obolibrary.org/obo/ENVO_00000004"/>
        <obo:RO_0001025 rdf:resource="http://purl.obolibrary.org/obo/GAZ_00014877"/>
        <obo:IAO_0000115>A sum (district) of Zavkhan Province in western Mongolia.</obo:IAO_0000115>
        <oboInOwl:hasOBONamespace>GAZ</oboInOwl:hasOBONamespace>
        <oboInOwl:id>GAZ:00027387</oboInOwl:id>
        <rdfs:label>Nomrog District</rdfs:label>
    </owl:NamedIndividual>
    


    <!-- http://purl.obolibrary.org/obo/GAZ_00027388 -->

    <owl:NamedIndividual rdf:about="http://purl.obolibrary.org/obo/GAZ_00027388">
        <rdf:type rdf:resource="http://purl.obolibrary.org/obo/ENVO_00000004"/>
        <obo:RO_0001025 rdf:resource="http://purl.obolibrary.org/obo/GAZ_00014877"/>
        <obo:IAO_0000115>A sum (district) of Zavkhan Province in western Mongolia.</obo:IAO_0000115>
        <oboInOwl:hasOBONamespace>GAZ</oboInOwl:hasOBONamespace>
        <oboInOwl:id>GAZ:00027388</oboInOwl:id>
        <rdfs:label>Santmargats District</rdfs:label>
    </owl:NamedIndividual>
    


    <!-- http://purl.obolibrary.org/obo/GAZ_00027389 -->

    <owl:NamedIndividual rdf:about="http://purl.obolibrary.org/obo/GAZ_00027389">
        <rdf:type rdf:resource="http://purl.obolibrary.org/obo/ENVO_00000004"/>
        <obo:RO_0001025 rdf:resource="http://purl.obolibrary.org/obo/GAZ_00014877"/>
        <obo:IAO_0000115>A sum (district) of Zavkhan Province in western Mongolia.</obo:IAO_0000115>
        <oboInOwl:hasOBONamespace>GAZ</oboInOwl:hasOBONamespace>
        <oboInOwl:id>GAZ:00027389</oboInOwl:id>
        <rdfs:label>Erdenekhairkhan District</rdfs:label>
    </owl:NamedIndividual>
    


    <!-- http://purl.obolibrary.org/obo/GAZ_00027390 -->

    <owl:NamedIndividual rdf:about="http://purl.obolibrary.org/obo/GAZ_00027390">
        <rdf:type rdf:resource="http://purl.obolibrary.org/obo/ENVO_00000004"/>
        <obo:RO_0001025 rdf:resource="http://purl.obolibrary.org/obo/GAZ_00014877"/>
        <obo:IAO_0000115>A sum (district) of Zavkhan Province in western Mongolia.</obo:IAO_0000115>
        <oboInOwl:hasOBONamespace>GAZ</oboInOwl:hasOBONamespace>
        <oboInOwl:id>GAZ:00027390</oboInOwl:id>
        <rdfs:label>Bayankhairkhan District</rdfs:label>
    </owl:NamedIndividual>
    


    <!-- http://purl.obolibrary.org/obo/GAZ_00027391 -->

    <owl:NamedIndividual rdf:about="http://purl.obolibrary.org/obo/GAZ_00027391">
        <rdf:type rdf:resource="http://purl.obolibrary.org/obo/ENVO_00000004"/>
        <obo:RO_0001025 rdf:resource="http://purl.obolibrary.org/obo/GAZ_00014877"/>
        <obo:IAO_0000115>A sum (district) of Zavkhan Province in western Mongolia.</obo:IAO_0000115>
        <oboInOwl:hasOBONamespace>GAZ</oboInOwl:hasOBONamespace>
        <oboInOwl:id>GAZ:00027391</oboInOwl:id>
        <rdfs:label>Tsetsen-Uul District</rdfs:label>
    </owl:NamedIndividual>
    


    <!-- http://purl.obolibrary.org/obo/GAZ_00027392 -->

    <owl:NamedIndividual rdf:about="http://purl.obolibrary.org/obo/GAZ_00027392">
        <rdf:type rdf:resource="http://purl.obolibrary.org/obo/ENVO_00000004"/>
        <obo:RO_0001025 rdf:resource="http://purl.obolibrary.org/obo/GAZ_00014877"/>
        <obo:IAO_0000115>A sum (district) of Zavkhan Province in western Mongolia.</obo:IAO_0000115>
        <oboInOwl:hasOBONamespace>GAZ</oboInOwl:hasOBONamespace>
        <oboInOwl:id>GAZ:00027392</oboInOwl:id>
        <rdfs:label>Bayantes District</rdfs:label>
    </owl:NamedIndividual>
    


    <!-- http://purl.obolibrary.org/obo/GAZ_00027393 -->

    <owl:NamedIndividual rdf:about="http://purl.obolibrary.org/obo/GAZ_00027393">
        <rdf:type rdf:resource="http://purl.obolibrary.org/obo/ENVO_00000004"/>
        <obo:RO_0001025 rdf:resource="http://purl.obolibrary.org/obo/GAZ_00014877"/>
        <obo:IAO_0000115>A sum (district) of Zavkhan Province in western Mongolia.</obo:IAO_0000115>
        <oboInOwl:hasOBONamespace>GAZ</oboInOwl:hasOBONamespace>
        <oboInOwl:id>GAZ:00027393</oboInOwl:id>
        <rdfs:label>Telmen District</rdfs:label>
    </owl:NamedIndividual>
    


    <!-- http://purl.obolibrary.org/obo/GAZ_00027394 -->

    <owl:NamedIndividual rdf:about="http://purl.obolibrary.org/obo/GAZ_00027394">
        <rdf:type rdf:resource="http://purl.obolibrary.org/obo/ENVO_00000004"/>
        <obo:RO_0001025 rdf:resource="http://purl.obolibrary.org/obo/GAZ_00014877"/>
        <obo:IAO_0000115>A sum (district) of Zavkhan Province in western Mongolia.</obo:IAO_0000115>
        <oboInOwl:hasOBONamespace>GAZ</oboInOwl:hasOBONamespace>
        <oboInOwl:id>GAZ:00027394</oboInOwl:id>
        <rdfs:label>Songino District</rdfs:label>
    </owl:NamedIndividual>
    


    <!-- http://purl.obolibrary.org/obo/GAZ_00027395 -->

    <owl:NamedIndividual rdf:about="http://purl.obolibrary.org/obo/GAZ_00027395">
        <rdf:type rdf:resource="http://purl.obolibrary.org/obo/ENVO_00000004"/>
        <obo:RO_0001025 rdf:resource="http://purl.obolibrary.org/obo/GAZ_00014877"/>
        <obo:IAO_0000115>A sum (district) of Zavkhan Province in western Mongolia.</obo:IAO_0000115>
        <oboInOwl:hasOBONamespace>GAZ</oboInOwl:hasOBONamespace>
        <oboInOwl:id>GAZ:00027395</oboInOwl:id>
        <rdfs:label>Tosontsengel District</rdfs:label>
    </owl:NamedIndividual>
    


    <!-- http://purl.obolibrary.org/obo/GAZ_00054868 -->

    <owl:NamedIndividual rdf:about="http://purl.obolibrary.org/obo/GAZ_00054868">
        <obo:RO_0001025 rdf:resource="http://purl.obolibrary.org/obo/GAZ_00008744"/>
        <obo:IAO_0000115>A volcanic field that lies in north-central Mongolia about 250 km west of Ulaanbaatar. This area is located in a broad region of Miocene-to-Holocene basaltic lavas in the Baikal Rift System SSW of Lake Baikal. Lava flows of four Miocene-to-Holocene age groups form terraces along the Chulutu (Chuloot) River; Pleistocene basalts form the 40- to 60-m terrace of the Taryatu basin. Six Holocene cinder cones, including Khorog (Horog) and Dzan Tologai, are concentrated along the Sumein and Gichgeniyn river valleys at the western end of the volcanic field. The 180-m-wide crater of Khorog is breached to the south, in the direction of an associated lava flow. The Holocene cones produced thin, freshly preserved lava flows remarkable for their large numbers of ultramafic xenoliths. The lava flow from Khorog was radiocarbon dated at about 4930 years ago and dammed the Chulutu River, forming Lake Terkhin-Tsagan-Nur.</obo:IAO_0000115>
        <oboInOwl:hasOBONamespace>GAZ</oboInOwl:hasOBONamespace>
        <oboInOwl:id>GAZ:00054868</oboInOwl:id>
        <rdfs:label>Taryatu-Chulutu Volcanic Field</rdfs:label>
    </owl:NamedIndividual>
    


    <!-- http://purl.obolibrary.org/obo/GAZ_00054869 -->

    <owl:NamedIndividual rdf:about="http://purl.obolibrary.org/obo/GAZ_00054869">
        <obo:RO_0001025 rdf:resource="http://purl.obolibrary.org/obo/GAZ_00054868"/>
        <obo:IAO_0000115>A lake formed by the damming of the Chulutu River by a lava flow.</obo:IAO_0000115>
        <oboInOwl:hasOBONamespace>GAZ</oboInOwl:hasOBONamespace>
        <oboInOwl:id>GAZ:00054869</oboInOwl:id>
        <rdfs:label>Lake Terkhin-Tsagan-Nur</rdfs:label>
    </owl:NamedIndividual>
    


    <!-- http://purl.obolibrary.org/obo/GAZ_00054870 -->

    <owl:NamedIndividual rdf:about="http://purl.obolibrary.org/obo/GAZ_00054870">
        <obo:RO_0001025 rdf:resource="http://purl.obolibrary.org/obo/GAZ_00054868"/>
        <obo:IAO_0000115>A cinder cone.</obo:IAO_0000115>
        <oboInOwl:hasOBONamespace>GAZ</oboInOwl:hasOBONamespace>
        <oboInOwl:id>GAZ:00054870</oboInOwl:id>
        <rdfs:label>Khorog Volcano</rdfs:label>
    </owl:NamedIndividual>
    


    <!-- http://purl.obolibrary.org/obo/GAZ_00054871 -->

    <owl:NamedIndividual rdf:about="http://purl.obolibrary.org/obo/GAZ_00054871">
        <obo:RO_0001025 rdf:resource="http://purl.obolibrary.org/obo/GAZ_00054868"/>
        <obo:IAO_0000115>A cinder cone.</obo:IAO_0000115>
        <oboInOwl:hasOBONamespace>GAZ</oboInOwl:hasOBONamespace>
        <oboInOwl:id>GAZ:00054871</oboInOwl:id>
        <rdfs:label>Dzan Tologai Volcano</rdfs:label>
    </owl:NamedIndividual>
    


    <!-- http://purl.obolibrary.org/obo/GAZ_00054872 -->

    <owl:NamedIndividual rdf:about="http://purl.obolibrary.org/obo/GAZ_00054872">
        <obo:RO_0001025 rdf:resource="http://purl.obolibrary.org/obo/GAZ_00008744"/>
        <obo:IAO_0000115>A volcanic field that consists of a group of 10 olivine-basaltic lava and cinder cones in west-central Mongolia about 150 km WNW of the capital city of Ulaanbaatar. The volcanic field covers a 3500 km2 flat-lying plain along the Khanuy River and in drainages to the east. The cones, including the well-preserved Togo cones about 50 km east of Khanuy, north of the settlement of Bulgan, range from about 30 to 190 m in height. The Togo cones, rich in ilmenite megacrysts and altered peridotite xenoliths, include Ikh Togo Uul (&quot;Great Togo Mountain&quot;) and Baga Togo Uul &quot;Big Togo Mountain&apos;).</obo:IAO_0000115>
        <oboInOwl:hasOBONamespace>GAZ</oboInOwl:hasOBONamespace>
        <oboInOwl:id>GAZ:00054872</oboInOwl:id>
        <rdfs:label>Khanuy Gol Volcanic Field</rdfs:label>
    </owl:NamedIndividual>
    


    <!-- http://purl.obolibrary.org/obo/GAZ_00054873 -->

    <owl:NamedIndividual rdf:about="http://purl.obolibrary.org/obo/GAZ_00054873">
        <obo:RO_0001025 rdf:resource="http://purl.obolibrary.org/obo/GAZ_00008744"/>
        <obo:IAO_0000115>The valley of the f the Orkhon River in Central Mongolia. A World Heritage Site.</obo:IAO_0000115>
        <oboInOwl:hasOBONamespace>GAZ</oboInOwl:hasOBONamespace>
        <oboInOwl:id>GAZ:00054873</oboInOwl:id>
        <rdfs:label>Orkhon Valley</rdfs:label>
    </owl:NamedIndividual>
    


    <!-- http://purl.obolibrary.org/obo/GAZ_00054875 -->

    <owl:NamedIndividual rdf:about="http://purl.obolibrary.org/obo/GAZ_00054875">
        <obo:RO_0001025 rdf:resource="http://purl.obolibrary.org/obo/GAZ_00008744"/>
        <obo:IAO_0000115>A 90 m high basaltic cinder cone of possible late-Pleistocene to Holocene age located east of the Orchon Gol area of east-central Mongolia, about 100 km SE of the capital city of Ulaanbaatar.</obo:IAO_0000115>
        <oboInOwl:hasOBONamespace>GAZ</oboInOwl:hasOBONamespace>
        <oboInOwl:id>GAZ:00054875</oboInOwl:id>
        <rdfs:label>Bus-Obo Volcano</rdfs:label>
    </owl:NamedIndividual>
    


    <!-- http://purl.obolibrary.org/obo/GAZ_00054876 -->

    <owl:NamedIndividual rdf:about="http://purl.obolibrary.org/obo/GAZ_00054876">
        <obo:RO_0001025 rdf:resource="http://purl.obolibrary.org/obo/GAZ_00014887"/>
        <obo:IAO_0000115>A volcanic field, located in SE Mongolia near the China border, that consists of more than 200 lava and cinder cones of Pleistocene and Holocene age that were erupted from NE-trending parallel fissures. The cones range in height from 25 to 300 m, and vary from partially eroded to completely preserved. Compositionally the volcanic rocks are more soda-rich than the potassium-rich rocks of northern and central Mongolia and consist of basaltic, trachybasaltic, and foiditic rocks. The southern part of the volcanic field, which may be contiguous with the Dolon Nor volcanic field across the border in China, is rich in ultramafic xenoliths.</obo:IAO_0000115>
        <oboInOwl:hasOBONamespace>GAZ</oboInOwl:hasOBONamespace>
        <oboInOwl:id>GAZ:00054876</oboInOwl:id>
        <rdfs:label>Dariganga Volcanic Field</rdfs:label>
    </owl:NamedIndividual>
    


    <!-- http://purl.obolibrary.org/obo/GAZ_00054877 -->

    <owl:NamedIndividual rdf:about="http://purl.obolibrary.org/obo/GAZ_00054877">
        <obo:RO_0001025 rdf:resource="http://purl.obolibrary.org/obo/GAZ_00008744"/>
        <obo:IAO_0000115>A volcanic field that consists of three basaltic cinder cones in south-central Mongolia, about 150 km south of the capital city of Ulaanbaatar. The 60-80 m high cones were constructed along an E-W-trending fault and are possibly of late-Pleistocene to Holocene age.</obo:IAO_0000115>
        <oboInOwl:hasOBONamespace>GAZ</oboInOwl:hasOBONamespace>
        <oboInOwl:id>GAZ:00054877</oboInOwl:id>
        <rdfs:label>Middle Gobi Volcanic Field</rdfs:label>
    </owl:NamedIndividual>
    


    <!-- http://purl.obolibrary.org/obo/GAZ_00056879 -->

    <owl:NamedIndividual rdf:about="http://purl.obolibrary.org/obo/GAZ_00056879">
        <obo:IAO_0000115>A mountain range in the Southeastern part of Altai Mountains. The range stretches 130 km northeast from 49degN and 86degE towards the western extremity of the Sayan Mountains in 51deg60minN and 89degE.</obo:IAO_0000115>
        <oboInOwl:hasOBONamespace>GAZ</oboInOwl:hasOBONamespace>
        <oboInOwl:id>GAZ:00056879</oboInOwl:id>
        <rdfs:label>Saylyugem Mountains</rdfs:label>
    </owl:NamedIndividual>
    


    <!-- http://purl.obolibrary.org/obo/GAZ_00057398 -->

    <owl:NamedIndividual rdf:about="http://purl.obolibrary.org/obo/GAZ_00057398">
        <obo:IAO_0000115>A part of the Altay mountain range, straddling the border of Russia and Kazakhstan close to the region where their borders and those of China and Mongolia meet.</obo:IAO_0000115>
        <oboInOwl:hasOBONamespace>GAZ</oboInOwl:hasOBONamespace>
        <oboInOwl:id>GAZ:00057398</oboInOwl:id>
        <rdfs:label>Chuya Alps</rdfs:label>
    </owl:NamedIndividual>
    


    <!-- http://purl.obolibrary.org/obo/GAZ_00057445 -->

    <owl:NamedIndividual rdf:about="http://purl.obolibrary.org/obo/GAZ_00057445">
        <obo:IAO_0000115>An eroded plateau-type highland in the Southwestern Siberia, Russia, particularly in Altai Krai, Kemerovo and Novosibirsk Oblast. It is a natural continuation of Altai Mountains and separates the Kuznetsk Depression from the Ob Plain, the basin of Ob River. Its main ridge is nearly parallel to that of Kuznetsk Alatau. The ridge is some 300 km in length and 15-40 km wide. Major rivers include the Berd&apos;, Suenga River and Chumysh River.</obo:IAO_0000115>
        <oboInOwl:hasOBONamespace>GAZ</oboInOwl:hasOBONamespace>
        <oboInOwl:id>GAZ:00057445</oboInOwl:id>
        <rdfs:label>Salair Ridge</rdfs:label>
    </owl:NamedIndividual>
    


    <!-- http://purl.obolibrary.org/obo/GAZ_00057465 -->

    <owl:NamedIndividual rdf:about="http://purl.obolibrary.org/obo/GAZ_00057465">
        <obo:RO_0001025 rdf:resource="http://purl.obolibrary.org/obo/GAZ_00014882"/>
        <obo:RO_0001025 rdf:resource="http://purl.obolibrary.org/obo/GAZ_00057466"/>
        <obo:IAO_0000115>A mountain range in the Omnogovi Province of southern Mongolia. The range forms the eastern half of the Gobi Gurvansaikhan National Park.</obo:IAO_0000115>
        <oboInOwl:hasOBONamespace>GAZ</oboInOwl:hasOBONamespace>
        <oboInOwl:id>GAZ:00057465</oboInOwl:id>
        <rdfs:label>Gurvansaikhan Mountains</rdfs:label>
    </owl:NamedIndividual>
    


    <!-- http://purl.obolibrary.org/obo/GAZ_00057466 -->

    <owl:NamedIndividual rdf:about="http://purl.obolibrary.org/obo/GAZ_00057466">
        <obo:RO_0001025 rdf:resource="http://purl.obolibrary.org/obo/GAZ_00014882"/>
        <obo:IAO_0000115>A national park in southern Mongolia. The park lies on the northern edge of the Gobi desert. The higher elevations contain areas of steppe.</obo:IAO_0000115>
        <oboInOwl:hasOBONamespace>GAZ</oboInOwl:hasOBONamespace>
        <oboInOwl:id>GAZ:00057466</oboInOwl:id>
        <rdfs:label>Gobi Gurvansaikhan National Park</rdfs:label>
    </owl:NamedIndividual>
    


    <!-- http://purl.obolibrary.org/obo/GAZ_00057467 -->

    <owl:NamedIndividual rdf:about="http://purl.obolibrary.org/obo/GAZ_00057467">
        <obo:RO_0001025 rdf:resource="http://purl.obolibrary.org/obo/GAZ_00008744"/>
        <obo:IAO_0000115>The largest desert region in Asia. It covers area in China and southern Mongolia. The desert basins of the Gobi are bounded by the Altay Mountains and the grasslands and steppes of Mongolia on the north, by the Tibetan Plateau to the southwest, and by the North China Plain to the southeast. The Gobi measures over 1,500 km from southwest to northeast and 800 km from north to south. The desert is widest in the west, along the line joining the Baghrash Kol and the Lop Nor (87degE-89degE). It occupies an arc of land 1,295,000 km2 in area. The Gobi includes the long stretch of desert and semidesert country extending from the foot of the Pamirs, 77degE, to the Greater Khingan Mountains, 116degE-118degE, on the border of Manchuria; and from the foothills of the Altay, Sayan, and Yablonoi mountain ranges on the north to the Kunlun Shan, Altun Shan, and Qilian shan ranges, which form the northern edges of the Tibetan Plateau, on the south.</obo:IAO_0000115>
        <oboInOwl:hasOBONamespace>GAZ</oboInOwl:hasOBONamespace>
        <oboInOwl:id>GAZ:00057467</oboInOwl:id>
        <rdfs:label>Gobi Desert</rdfs:label>
    </owl:NamedIndividual>
    


    <!-- http://purl.obolibrary.org/obo/GAZ_00057469 -->

    <owl:NamedIndividual rdf:about="http://purl.obolibrary.org/obo/GAZ_00057469">
        <obo:RO_0001025 rdf:resource="http://purl.obolibrary.org/obo/GAZ_00057466"/>
        <obo:IAO_0000115>A sand dune system.</obo:IAO_0000115>
        <oboInOwl:hasOBONamespace>GAZ</oboInOwl:hasOBONamespace>
        <oboInOwl:id>GAZ:00057469</oboInOwl:id>
        <rdfs:label>Khongoryn Els</rdfs:label>
    </owl:NamedIndividual>
    


    <!-- http://purl.obolibrary.org/obo/GAZ_00057752 -->

    <owl:NamedIndividual rdf:about="http://purl.obolibrary.org/obo/GAZ_00057752">
        <obo:RO_0001025 rdf:resource="http://purl.obolibrary.org/obo/GAZ_00057467"/>
        <obo:IAO_0000115>A part of the Gobi Desert that occupies the space between the Tian Shan system on the north and the Nan-shan Mountains on the south, and is connected on the west with the Lop Desert.</obo:IAO_0000115>
        <oboInOwl:hasOBONamespace>GAZ</oboInOwl:hasOBONamespace>
        <oboInOwl:id>GAZ:00057752</oboInOwl:id>
        <rdfs:label>Hami Desert</rdfs:label>
    </owl:NamedIndividual>
    


    <!-- http://purl.obolibrary.org/obo/GAZ_00057823 -->

    <owl:NamedIndividual rdf:about="http://purl.obolibrary.org/obo/GAZ_00057823">
        <obo:RO_0001025 rdf:resource="http://purl.obolibrary.org/obo/GAZ_00090195"/>
        <obo:IAO_0000115>A freshwater lake located in the northwest of Mongolia near the border to Russia, at the foot of the eastern Sayan Mountains. It is 1,645 m above sea level, 136 km long and 262 m deep. Its watershed is relatively small, and it only has small tributaries. It is drained at the south end by the Egiin Gol, which connects to the Selenge and ultimately into Lake Baikal.</obo:IAO_0000115>
        <oboInOwl:hasOBONamespace>GAZ</oboInOwl:hasOBONamespace>
        <oboInOwl:id>GAZ:00057823</oboInOwl:id>
        <rdfs:label>Lake Khovsgol</rdfs:label>
    </owl:NamedIndividual>
    


    <!-- http://purl.obolibrary.org/obo/GAZ_00057827 -->

    <owl:NamedIndividual rdf:about="http://purl.obolibrary.org/obo/GAZ_00057827">
        <obo:RO_0001025 rdf:resource="http://purl.obolibrary.org/obo/GAZ_00027327"/>
        <obo:IAO_0000115>A lake in Mongolia.</obo:IAO_0000115>
        <oboInOwl:hasOBONamespace>GAZ</oboInOwl:hasOBONamespace>
        <oboInOwl:id>GAZ:00057827</oboInOwl:id>
        <rdfs:label>Hyargas Nuur</rdfs:label>
    </owl:NamedIndividual>
    


    <!-- http://purl.obolibrary.org/obo/GAZ_00057876 -->

    <owl:NamedIndividual rdf:about="http://purl.obolibrary.org/obo/GAZ_00057876">
        <obo:RO_0001025 rdf:resource="http://purl.obolibrary.org/obo/GAZ_00008744"/>
        <obo:IAO_0000115>A mountain range in central Mongolia, some 400 km west of Ulaanbaatar.</obo:IAO_0000115>
        <oboInOwl:hasOBONamespace>GAZ</oboInOwl:hasOBONamespace>
        <oboInOwl:id>GAZ:00057876</oboInOwl:id>
        <rdfs:label>Khangai Mountains</rdfs:label>
    </owl:NamedIndividual>
    


    <!-- http://purl.obolibrary.org/obo/GAZ_00057877 -->

    <owl:NamedIndividual rdf:about="http://purl.obolibrary.org/obo/GAZ_00057877">
        <obo:RO_0001025 rdf:resource="http://purl.obolibrary.org/obo/GAZ_00014868"/>
        <obo:RO_0001025 rdf:resource="http://purl.obolibrary.org/obo/GAZ_00252305"/>
        <obo:IAO_0000115>An endorheic saline lake. Located in the broad inter-montane depression between the Khangai and Gobi-Altai mountains, at the foot of the Khara-Argalintu ridge of the Gobi-Altai.</obo:IAO_0000115>
        <oboInOwl:hasOBONamespace>GAZ</oboInOwl:hasOBONamespace>
        <oboInOwl:id>GAZ:00057877</oboInOwl:id>
        <rdfs:label>Boon Tsagaan Nuur</rdfs:label>
    </owl:NamedIndividual>
    


    <!-- http://purl.obolibrary.org/obo/GAZ_00057878 -->

    <owl:NamedIndividual rdf:about="http://purl.obolibrary.org/obo/GAZ_00057878">
        <obo:RO_0001025 rdf:resource="http://purl.obolibrary.org/obo/GAZ_00014868"/>
        <obo:RO_0001025 rdf:resource="http://purl.obolibrary.org/obo/GAZ_00252305"/>
        <obo:IAO_0000115>An endorheic saline lake. Located at the foot of the Ikhe Bogd Uul massif, in the Gobi Valley of Lakes, 125 km south of Jargalan, Bayankhongor Province.</obo:IAO_0000115>
        <oboInOwl:hasOBONamespace>GAZ</oboInOwl:hasOBONamespace>
        <oboInOwl:id>GAZ:00057878</oboInOwl:id>
        <rdfs:label>Orog Nuur</rdfs:label>
    </owl:NamedIndividual>
    


    <!-- http://purl.obolibrary.org/obo/GAZ_00057909 -->

    <owl:NamedIndividual rdf:about="http://purl.obolibrary.org/obo/GAZ_00057909">
        <obo:RO_0001025 rdf:resource="http://purl.obolibrary.org/obo/GAZ_00057910"/>
        <obo:IAO_0000115>A highly saline lake in an endorheic basin in Mongolia with a small part in Russia. The northeastern tip of the lake is situated in the Tuva Republic of the Russian Federation. The largest settlement near the lake is Ulaangom.</obo:IAO_0000115>
        <oboInOwl:hasOBONamespace>GAZ</oboInOwl:hasOBONamespace>
        <oboInOwl:id>GAZ:00057909</oboInOwl:id>
        <rdfs:label>Uvs Nuur</rdfs:label>
    </owl:NamedIndividual>
    


    <!-- http://purl.obolibrary.org/obo/GAZ_00057910 -->

    <owl:NamedIndividual rdf:about="http://purl.obolibrary.org/obo/GAZ_00057910">
        <obo:RO_0001025 rdf:resource="http://purl.obolibrary.org/obo/GAZ_00014876"/>
        <obo:IAO_0000115>A mountain endorheic basin, named after lake Uvs Nuur, a large, shallow and very saline lake in the basin&apos;s center.</obo:IAO_0000115>
        <oboInOwl:hasOBONamespace>GAZ</oboInOwl:hasOBONamespace>
        <oboInOwl:id>GAZ:00057910</oboInOwl:id>
        <rdfs:label>Uvs Nuur Basin</rdfs:label>
    </owl:NamedIndividual>
    


    <!-- http://purl.obolibrary.org/obo/GAZ_00057911 -->

    <owl:NamedIndividual rdf:about="http://purl.obolibrary.org/obo/GAZ_00057911">
        <obo:RO_0001025 rdf:resource="http://purl.obolibrary.org/obo/GAZ_00057910"/>
        <obo:IAO_0000115>A World Heritage Site. A fragile mountain hollow or depression located on the territorial border of Mongolia and the Republic of Tuva in the Russian Federation among the mountains, Tannu-Ola Mountains, and the Altay Mountains region, part of a combination of raised lands and depressions. Here the world&apos;s most northern desert meets the world&apos;s most southern tundra zone.</obo:IAO_0000115>
        <oboInOwl:hasOBONamespace>GAZ</oboInOwl:hasOBONamespace>
        <oboInOwl:id>GAZ:00057911</oboInOwl:id>
        <rdfs:label>Ubsunur Hollow Biosphere Reserve</rdfs:label>
    </owl:NamedIndividual>
    


    <!-- http://purl.obolibrary.org/obo/GAZ_00057934 -->

    <owl:NamedIndividual rdf:about="http://purl.obolibrary.org/obo/GAZ_00057934">
        <obo:RO_0001025 rdf:resource="http://purl.obolibrary.org/obo/GAZ_00150545"/>
        <obo:IAO_0000115>The largest lake in the Altay Mountains and the Altai Republic.</obo:IAO_0000115>
        <oboInOwl:hasOBONamespace>GAZ</oboInOwl:hasOBONamespace>
        <oboInOwl:id>GAZ:00057934</oboInOwl:id>
        <rdfs:label>Lake Teletskoye</rdfs:label>
    </owl:NamedIndividual>
    


    <!-- http://purl.obolibrary.org/obo/GAZ_00058407 -->

    <owl:NamedIndividual rdf:about="http://purl.obolibrary.org/obo/GAZ_00058407">
        <obo:RO_0001025 rdf:resource="http://purl.obolibrary.org/obo/GAZ_00117540"/>
        <obo:IAO_0000115>A freshwater lake in the Uvs Province of Mongolia, in the west of the country.</obo:IAO_0000115>
        <oboInOwl:hasOBONamespace>GAZ</oboInOwl:hasOBONamespace>
        <oboInOwl:id>GAZ:00058407</oboInOwl:id>
        <rdfs:label>Achit Nuur</rdfs:label>
    </owl:NamedIndividual>
    


    <!-- http://purl.obolibrary.org/obo/GAZ_00058408 -->

    <owl:NamedIndividual rdf:about="http://purl.obolibrary.org/obo/GAZ_00058408">
        <obo:RO_0001025 rdf:resource="http://purl.obolibrary.org/obo/GAZ_00027234"/>
        <obo:RO_0001025 rdf:resource="http://purl.obolibrary.org/obo/GAZ_00027256"/>
        <obo:RO_0001025 rdf:resource="http://purl.obolibrary.org/obo/GAZ_00027259"/>
        <obo:RO_0001025 rdf:resource="http://purl.obolibrary.org/obo/GAZ_00117527"/>
        <obo:IAO_0000115>A lake in northwestern Khovsgol Province, Mongolia, between the Tsagaannuur and Renchinlkhumbe sums. It is sometimes divided into the Targan, Dund, and Kharmai lakes. Targan nuur is 3.5 meters deep, Dund nuur 5 meters and Kharmai nuur 15 meters.</obo:IAO_0000115>
        <oboInOwl:hasOBONamespace>GAZ</oboInOwl:hasOBONamespace>
        <oboInOwl:id>GAZ:00058408</oboInOwl:id>
        <rdfs:label>Dood Tsagaan Nuur</rdfs:label>
    </owl:NamedIndividual>
    


    <!-- http://purl.obolibrary.org/obo/GAZ_00058409 -->

    <owl:NamedIndividual rdf:about="http://purl.obolibrary.org/obo/GAZ_00058409">
        <obo:RO_0001025 rdf:resource="http://purl.obolibrary.org/obo/GAZ_00058408"/>
        <obo:IAO_0000115>A part of Dood Tsagaan Nuur.</obo:IAO_0000115>
        <oboInOwl:hasOBONamespace>GAZ</oboInOwl:hasOBONamespace>
        <oboInOwl:id>GAZ:00058409</oboInOwl:id>
        <rdfs:label>Dund Nuur</rdfs:label>
    </owl:NamedIndividual>
    


    <!-- http://purl.obolibrary.org/obo/GAZ_00058410 -->

    <owl:NamedIndividual rdf:about="http://purl.obolibrary.org/obo/GAZ_00058410">
        <obo:RO_0001025 rdf:resource="http://purl.obolibrary.org/obo/GAZ_00058408"/>
        <obo:IAO_0000115>A part of Dood Tsagaan Nuur.</obo:IAO_0000115>
        <oboInOwl:hasOBONamespace>GAZ</oboInOwl:hasOBONamespace>
        <oboInOwl:id>GAZ:00058410</oboInOwl:id>
        <rdfs:label>Targan Nuur</rdfs:label>
    </owl:NamedIndividual>
    


    <!-- http://purl.obolibrary.org/obo/GAZ_00058411 -->

    <owl:NamedIndividual rdf:about="http://purl.obolibrary.org/obo/GAZ_00058411">
        <obo:RO_0001025 rdf:resource="http://purl.obolibrary.org/obo/GAZ_00058408"/>
        <obo:IAO_0000115>A part of Dood Tsagaan Nuur.</obo:IAO_0000115>
        <oboInOwl:hasOBONamespace>GAZ</oboInOwl:hasOBONamespace>
        <oboInOwl:id>GAZ:00058411</oboInOwl:id>
        <rdfs:label>Kharmai Nuur</rdfs:label>
    </owl:NamedIndividual>
    


    <!-- http://purl.obolibrary.org/obo/GAZ_00058413 -->

    <owl:NamedIndividual rdf:about="http://purl.obolibrary.org/obo/GAZ_00058413">
        <obo:IAO_0000115>A saline lake.</obo:IAO_0000115>
        <oboInOwl:hasOBONamespace>GAZ</oboInOwl:hasOBONamespace>
        <oboInOwl:id>GAZ:00058413</oboInOwl:id>
        <rdfs:label>Khyargas Nuur</rdfs:label>
    </owl:NamedIndividual>
    


    <!-- http://purl.obolibrary.org/obo/GAZ_00058414 -->

    <owl:NamedIndividual rdf:about="http://purl.obolibrary.org/obo/GAZ_00058414">
        <obo:IAO_0000115>A freshwater lake located in western Mongolia&apos;s Great Lakes Depression. It is part of a group of lakes that were once part of a larger prehistoric lake that disappeared 5,000 years ago as the region became drier. The lake is connected to Khar-Us Nuur to the east by the Conoharayh Gol.</obo:IAO_0000115>
        <oboInOwl:hasOBONamespace>GAZ</oboInOwl:hasOBONamespace>
        <oboInOwl:id>GAZ:00058414</oboInOwl:id>
        <rdfs:label>Khar Nuur</rdfs:label>
    </owl:NamedIndividual>
    


    <!-- http://purl.obolibrary.org/obo/GAZ_00058415 -->

    <owl:NamedIndividual rdf:about="http://purl.obolibrary.org/obo/GAZ_00058415">
        <obo:IAO_0000115>A freshwater lake in western Mongolia in the Great Lakes Depression. It is the upper one in a system of the interconnected lakes: Khar-Us Nuur, Khar Nuur, Dorgon Nuur, Airag Nuur and Khyargas Nuur. Primary inflow is the Khovd Gol river, which creates a large river delta. The lake is connected to Khar Nuur to the east by the Conoharayh Gol.</obo:IAO_0000115>
        <oboInOwl:hasOBONamespace>GAZ</oboInOwl:hasOBONamespace>
        <oboInOwl:id>GAZ:00058415</oboInOwl:id>
        <rdfs:label>Khar-Us Nuur</rdfs:label>
    </owl:NamedIndividual>
    


    <!-- http://purl.obolibrary.org/obo/GAZ_00058416 -->

    <owl:NamedIndividual rdf:about="http://purl.obolibrary.org/obo/GAZ_00058416">
        <obo:RO_0001025 rdf:resource="http://purl.obolibrary.org/obo/GAZ_00026088"/>
        <obo:IAO_0000115>A small freshwater lake in the Arkhangai Province in central Mongolia. Located the valley of the Orkhon River, to the north of the main Khangai ridge in the Arctic Ocean Drainage Basin,165 km north of Arvayheer.</obo:IAO_0000115>
        <oboInOwl:hasOBONamespace>GAZ</oboInOwl:hasOBONamespace>
        <oboInOwl:id>GAZ:00058416</oboInOwl:id>
        <rdfs:label>Ogii Nuur</rdfs:label>
    </owl:NamedIndividual>
    


    <!-- http://purl.obolibrary.org/obo/GAZ_00058417 -->

    <owl:NamedIndividual rdf:about="http://purl.obolibrary.org/obo/GAZ_00058417">
        <obo:RO_0001025 rdf:resource="http://purl.obolibrary.org/obo/GAZ_00014877"/>
        <obo:IAO_0000115>A lake in Dzavhan, in Zavkhan Aimag in north-west Mongolia.</obo:IAO_0000115>
        <oboInOwl:hasOBONamespace>GAZ</oboInOwl:hasOBONamespace>
        <oboInOwl:id>GAZ:00058417</oboInOwl:id>
        <rdfs:label>Oigon Nuur</rdfs:label>
    </owl:NamedIndividual>
    


    <!-- http://purl.obolibrary.org/obo/GAZ_00058418 -->

    <owl:NamedIndividual rdf:about="http://purl.obolibrary.org/obo/GAZ_00058418">
        <obo:RO_0001025 rdf:resource="http://purl.obolibrary.org/obo/GAZ_00027227"/>
        <obo:RO_0001025 rdf:resource="http://purl.obolibrary.org/obo/GAZ_00027235"/>
        <obo:RO_0001025 rdf:resource="http://purl.obolibrary.org/obo/GAZ_00027247"/>
        <obo:RO_0001025 rdf:resource="http://purl.obolibrary.org/obo/GAZ_00027378"/>
        <obo:IAO_0000115>A saline lake in northern Mongolia, located at the border between the Tsagaan-Uul, Shine-Ider, and Burentogtokh sums of Khovsgol Province, and the Ikh-Uul sum of Zavkhan Province.</obo:IAO_0000115>
        <oboInOwl:hasOBONamespace>GAZ</oboInOwl:hasOBONamespace>
        <oboInOwl:id>GAZ:00058418</oboInOwl:id>
        <rdfs:label>Sangiin Dalai Nuur</rdfs:label>
    </owl:NamedIndividual>
    


    <!-- http://purl.obolibrary.org/obo/GAZ_00058419 -->

    <owl:NamedIndividual rdf:about="http://purl.obolibrary.org/obo/GAZ_00058419">
        <obo:RO_0001025 rdf:resource="http://purl.obolibrary.org/obo/GAZ_00057876"/>
        <obo:RO_0001025 rdf:resource="http://purl.obolibrary.org/obo/GAZ_00090201"/>
        <obo:IAO_0000115>A freshwater lake in the Khangai Mountains in central Mongolia. The Khorgo volcano is located near the eastern end of the lake and the Suman gol river springs from lake.</obo:IAO_0000115>
        <oboInOwl:hasOBONamespace>GAZ</oboInOwl:hasOBONamespace>
        <oboInOwl:id>GAZ:00058419</oboInOwl:id>
        <rdfs:label>Terkhiin Tsagaan Nuur</rdfs:label>
    </owl:NamedIndividual>
    


    <!-- http://purl.obolibrary.org/obo/GAZ_00090194 -->

    <owl:NamedIndividual rdf:about="http://purl.obolibrary.org/obo/GAZ_00090194">
        <obo:IAO_0000115>A national park. Established 1993.</obo:IAO_0000115>
        <oboInOwl:hasOBONamespace>GAZ</oboInOwl:hasOBONamespace>
        <oboInOwl:id>GAZ:00090194</oboInOwl:id>
        <rdfs:label>Gorkhi-Terelj National Park</rdfs:label>
    </owl:NamedIndividual>
    


    <!-- http://purl.obolibrary.org/obo/GAZ_00090195 -->

    <owl:NamedIndividual rdf:about="http://purl.obolibrary.org/obo/GAZ_00090195">
        <obo:RO_0001025 rdf:resource="http://purl.obolibrary.org/obo/GAZ_00014885"/>
        <obo:IAO_0000115>A national park.</obo:IAO_0000115>
        <oboInOwl:hasOBONamespace>GAZ</oboInOwl:hasOBONamespace>
        <oboInOwl:id>GAZ:00090195</oboInOwl:id>
        <rdfs:label>Lake Khovsgol National Park</rdfs:label>
    </owl:NamedIndividual>
    


    <!-- http://purl.obolibrary.org/obo/GAZ_00090196 -->

    <owl:NamedIndividual rdf:about="http://purl.obolibrary.org/obo/GAZ_00090196">
        <obo:RO_0001025 rdf:resource="http://purl.obolibrary.org/obo/GAZ_00008744"/>
        <obo:IAO_0000115>A national park in Mongolia.</obo:IAO_0000115>
        <oboInOwl:hasOBONamespace>GAZ</oboInOwl:hasOBONamespace>
        <oboInOwl:id>GAZ:00090196</oboInOwl:id>
        <rdfs:label>Southern Altai Gobi National Park</rdfs:label>
    </owl:NamedIndividual>
    


    <!-- http://purl.obolibrary.org/obo/GAZ_00090197 -->

    <owl:NamedIndividual rdf:about="http://purl.obolibrary.org/obo/GAZ_00090197">
        <obo:RO_0001025 rdf:resource="http://purl.obolibrary.org/obo/GAZ_00014878"/>
        <obo:IAO_0000115>A national park in Mongolia.</obo:IAO_0000115>
        <oboInOwl:hasOBONamespace>GAZ</oboInOwl:hasOBONamespace>
        <oboInOwl:id>GAZ:00090197</oboInOwl:id>
        <rdfs:label>Tsambagarav Lul National Park</rdfs:label>
    </owl:NamedIndividual>
    


    <!-- http://purl.obolibrary.org/obo/GAZ_00090198 -->

    <owl:NamedIndividual rdf:about="http://purl.obolibrary.org/obo/GAZ_00090198">
        <obo:RO_0001025 rdf:resource="http://purl.obolibrary.org/obo/GAZ_00014878"/>
        <obo:IAO_0000115>A national park in Mongolia.</obo:IAO_0000115>
        <oboInOwl:hasOBONamespace>GAZ</oboInOwl:hasOBONamespace>
        <oboInOwl:id>GAZ:00090198</oboInOwl:id>
        <rdfs:label>Tavan Bogd National Park</rdfs:label>
    </owl:NamedIndividual>
    


    <!-- http://purl.obolibrary.org/obo/GAZ_00090199 -->

    <owl:NamedIndividual rdf:about="http://purl.obolibrary.org/obo/GAZ_00090199">
        <obo:IAO_0000115>A national park in Mongolia.</obo:IAO_0000115>
        <oboInOwl:hasOBONamespace>GAZ</oboInOwl:hasOBONamespace>
        <oboInOwl:id>GAZ:00090199</oboInOwl:id>
        <rdfs:label>Khan Khentii Strictly Protected Area</rdfs:label>
    </owl:NamedIndividual>
    


    <!-- http://purl.obolibrary.org/obo/GAZ_00090200 -->

    <owl:NamedIndividual rdf:about="http://purl.obolibrary.org/obo/GAZ_00090200">
        <obo:RO_0001025 rdf:resource="http://purl.obolibrary.org/obo/GAZ_00014869"/>
        <obo:IAO_0000115>A national park in Mongolia.</obo:IAO_0000115>
        <oboInOwl:hasOBONamespace>GAZ</oboInOwl:hasOBONamespace>
        <oboInOwl:id>GAZ:00090200</oboInOwl:id>
        <rdfs:label>Khustain Nuruu National Park</rdfs:label>
    </owl:NamedIndividual>
    


    <!-- http://purl.obolibrary.org/obo/GAZ_00090201 -->

    <owl:NamedIndividual rdf:about="http://purl.obolibrary.org/obo/GAZ_00090201">
        <obo:RO_0001025 rdf:resource="http://purl.obolibrary.org/obo/GAZ_00014880"/>
        <obo:IAO_0000115>A national park in Mongolia.</obo:IAO_0000115>
        <oboInOwl:hasOBONamespace>GAZ</oboInOwl:hasOBONamespace>
        <oboInOwl:id>GAZ:00090201</oboInOwl:id>
        <rdfs:label>Khorgo-Terkhiin Tsagaan Nuur National Park</rdfs:label>
    </owl:NamedIndividual>
    


    <!-- http://purl.obolibrary.org/obo/GAZ_00114665 -->

    <owl:NamedIndividual rdf:about="http://purl.obolibrary.org/obo/GAZ_00114665">
        <obo:RO_0001025 rdf:resource="http://purl.obolibrary.org/obo/GAZ_00057467"/>
        <obo:IAO_0000115>A basin in the Autonomous Region of Xinjiang in northwestern China. It is surrounded by mountains. The basin is located between the Mongolian Altai Mountains and Tian Shan to the north. The basin is similar to the larger Tarim Basin on the southern side of the Tian Shan Range.</obo:IAO_0000115>
        <oboInOwl:hasOBONamespace>GAZ</oboInOwl:hasOBONamespace>
        <oboInOwl:id>GAZ:00114665</oboInOwl:id>
        <rdfs:label>Dzungaria Basin</rdfs:label>
    </owl:NamedIndividual>
    


    <!-- http://purl.obolibrary.org/obo/GAZ_00114666 -->

    <owl:NamedIndividual rdf:about="http://purl.obolibrary.org/obo/GAZ_00114666">
        <obo:RO_0001025 rdf:resource="http://purl.obolibrary.org/obo/GAZ_00114665"/>
        <obo:IAO_0000115>A desert located in the center of the Dzungaria Basin.</obo:IAO_0000115>
        <oboInOwl:hasOBONamespace>GAZ</oboInOwl:hasOBONamespace>
        <oboInOwl:id>GAZ:00114666</oboInOwl:id>
        <rdfs:label>Gurbantunggut Desert</rdfs:label>
    </owl:NamedIndividual>
    


    <!-- http://purl.obolibrary.org/obo/GAZ_00117271 -->

    <owl:NamedIndividual rdf:about="http://purl.obolibrary.org/obo/GAZ_00117271">
        <obo:RO_0001025 rdf:resource="http://purl.obolibrary.org/obo/GAZ_00114665"/>
        <obo:IAO_0000115>A saline lake. Located on the extreme southeastern edge of the Junggar Basin, west of the town of Barkol, 100 km northwest of Hami, Xinjiang Zizhiqu.</obo:IAO_0000115>
        <oboInOwl:hasOBONamespace>GAZ</oboInOwl:hasOBONamespace>
        <oboInOwl:id>GAZ:00117271</oboInOwl:id>
        <rdfs:label>Barkol Hu</rdfs:label>
    </owl:NamedIndividual>
    


    <!-- http://purl.obolibrary.org/obo/GAZ_00117273 -->

    <owl:NamedIndividual rdf:about="http://purl.obolibrary.org/obo/GAZ_00117273">
        <obo:RO_0001025 rdf:resource="http://purl.obolibrary.org/obo/GAZ_00114665"/>
        <obo:IAO_0000115>A now-dry saline lake in a closed sub-basin in the central part of the Zhungeer (Zhunggar) Basin, western Xinjiang. The Zhungeer Basin is bordered to the north by the Altai Mountains (Altai Shan), to the south by the Tian Mountains (Tian Shan), and to the west by a series of mountains and plateaus that rise to elevations of ca 3000 m. The former lake bed is now covered by a halite crust.</obo:IAO_0000115>
        <oboInOwl:hasOBONamespace>GAZ</oboInOwl:hasOBONamespace>
        <oboInOwl:id>GAZ:00117273</oboInOwl:id>
        <rdfs:label>Manasi Hu</rdfs:label>
    </owl:NamedIndividual>
    


    <!-- http://purl.obolibrary.org/obo/GAZ_00117274 -->

    <owl:NamedIndividual rdf:about="http://purl.obolibrary.org/obo/GAZ_00117274">
        <obo:RO_0001025 rdf:resource="http://purl.obolibrary.org/obo/GAZ_00057467"/>
        <obo:IAO_0000115>A saline lake in the Eastern Gobi Desert.</obo:IAO_0000115>
        <oboInOwl:hasOBONamespace>GAZ</oboInOwl:hasOBONamespace>
        <oboInOwl:id>GAZ:00117274</oboInOwl:id>
        <rdfs:label>Taboos-nor</rdfs:label>
    </owl:NamedIndividual>
    


    <!-- http://purl.obolibrary.org/obo/GAZ_00117518 -->

    <owl:NamedIndividual rdf:about="http://purl.obolibrary.org/obo/GAZ_00117518">
        <obo:RO_0001025 rdf:resource="http://purl.obolibrary.org/obo/GAZ_00027124"/>
        <obo:IAO_0000115>A national protected area in the Bulgan Province of Mongolia. It is located about 60km directly west of Bulgan city around the extinct volcanoes Uran Togoo, Tulga Togoo, and Jalavch Uul.</obo:IAO_0000115>
        <oboInOwl:hasOBONamespace>GAZ</oboInOwl:hasOBONamespace>
        <oboInOwl:id>GAZ:00117518</oboInOwl:id>
        <rdfs:label>Uran-Togoo Tulga Uul Natural Monument</rdfs:label>
    </owl:NamedIndividual>
    


    <!-- http://purl.obolibrary.org/obo/GAZ_00117519 -->

    <owl:NamedIndividual rdf:about="http://purl.obolibrary.org/obo/GAZ_00117519">
        <obo:IAO_0000115>A freshwater lake.</obo:IAO_0000115>
        <oboInOwl:hasOBONamespace>GAZ</oboInOwl:hasOBONamespace>
        <oboInOwl:id>GAZ:00117519</oboInOwl:id>
        <rdfs:label>Airag Nuur</rdfs:label>
    </owl:NamedIndividual>
    


    <!-- http://purl.obolibrary.org/obo/GAZ_00117520 -->

    <owl:NamedIndividual rdf:about="http://purl.obolibrary.org/obo/GAZ_00117520">
        <obo:IAO_0000115>A saline lake. It is connected to Khar Nuur to the northwest by the Homin Holoy River.</obo:IAO_0000115>
        <oboInOwl:hasOBONamespace>GAZ</oboInOwl:hasOBONamespace>
        <oboInOwl:id>GAZ:00117520</oboInOwl:id>
        <rdfs:label>Dorgon Nuur</rdfs:label>
    </owl:NamedIndividual>
    


    <!-- http://purl.obolibrary.org/obo/GAZ_00117521 -->

    <owl:NamedIndividual rdf:about="http://purl.obolibrary.org/obo/GAZ_00117521">
        <obo:RO_0001025 rdf:resource="http://purl.obolibrary.org/obo/GAZ_00014882"/>
        <obo:IAO_0000115>A basin situated in the northwestern part of the Gobi Desert, in the Omnogovi Province in the southern part of Mongolia.</obo:IAO_0000115>
        <oboInOwl:hasOBONamespace>GAZ</oboInOwl:hasOBONamespace>
        <oboInOwl:id>GAZ:00117521</oboInOwl:id>
        <rdfs:label>Nemegt Basin</rdfs:label>
    </owl:NamedIndividual>
    


    <!-- http://purl.obolibrary.org/obo/GAZ_00117522 -->

    <owl:NamedIndividual rdf:about="http://purl.obolibrary.org/obo/GAZ_00117522">
        <obo:RO_0001025 rdf:resource="http://purl.obolibrary.org/obo/GAZ_00014871"/>
        <obo:IAO_0000115>A depression near Choir, Mongolia. It is about 150 km long and 10 to 20 km wide, about 500 m lower than the surrounding upland. It lies at an altitude of 1269 m.</obo:IAO_0000115>
        <oboInOwl:hasOBONamespace>GAZ</oboInOwl:hasOBONamespace>
        <oboInOwl:id>GAZ:00117522</oboInOwl:id>
        <rdfs:label>Choir Depression</rdfs:label>
    </owl:NamedIndividual>
    


    <!-- http://purl.obolibrary.org/obo/GAZ_00117523 -->

    <owl:NamedIndividual rdf:about="http://purl.obolibrary.org/obo/GAZ_00117523">
        <obo:RO_0001025 rdf:resource="http://purl.obolibrary.org/obo/GAZ_00014870"/>
        <obo:IAO_0000115>A meteorite crater in the Dornogovi Aimag (province) the south-east of Mongolia. The crater, which is exposed at the surface, is 1.3 km in diameter and has an estimated age of 150 +/- 20 million years (Upper Jurassic).</obo:IAO_0000115>
        <oboInOwl:hasOBONamespace>GAZ</oboInOwl:hasOBONamespace>
        <oboInOwl:id>GAZ:00117523</oboInOwl:id>
        <rdfs:label>Tabun-Khara-Obo Crater</rdfs:label>
    </owl:NamedIndividual>
    


    <!-- http://purl.obolibrary.org/obo/GAZ_00117524 -->

    <owl:NamedIndividual rdf:about="http://purl.obolibrary.org/obo/GAZ_00117524">
        <obo:RO_0001025 rdf:resource="http://purl.obolibrary.org/obo/GAZ_00090201"/>
        <obo:IAO_0000115>An extinct volcano in the Arkhangai Province of Mongolia. It is located on the northern slopes of the Khangai Mountains. The Khorgo lies east of the lake Terkhiin Tsagaan Nuur and together they are the core of the Khorgo-Terkhiin Tsagaan Nuur National Park.</obo:IAO_0000115>
        <oboInOwl:hasOBONamespace>GAZ</oboInOwl:hasOBONamespace>
        <oboInOwl:id>GAZ:00117524</oboInOwl:id>
        <rdfs:label>Khorgo</rdfs:label>
    </owl:NamedIndividual>
    


    <!-- http://purl.obolibrary.org/obo/GAZ_00117525 -->

    <owl:NamedIndividual rdf:about="http://purl.obolibrary.org/obo/GAZ_00117525">
        <rdf:type rdf:resource="http://purl.obolibrary.org/obo/ENVO_00000100"/>
        <rdf:type rdf:resource="http://purl.obolibrary.org/obo/ENVO_00000275"/>
        <obo:RO_0001025 rdf:resource="http://purl.obolibrary.org/obo/GAZ_00057465"/>
        <obo:IAO_0000115>A deep and narrow gorge in the Gurvansaikhan Mountains of southern Mongolia. Yolyn Am is found in the Zuun Saikhanii Nuruu (the Eastern Beauty) subrange of the Gurvansaikhan Mountains. The area, as part of the Gobi Desert, sees little precipitation. However, Yolyn Am is notable for a deep ice field.</obo:IAO_0000115>
        <oboInOwl:hasOBONamespace>GAZ</oboInOwl:hasOBONamespace>
        <oboInOwl:id>GAZ:00117525</oboInOwl:id>
        <rdfs:label>Yolyn Am</rdfs:label>
    </owl:NamedIndividual>
    


    <!-- http://purl.obolibrary.org/obo/GAZ_00117526 -->

    <owl:NamedIndividual rdf:about="http://purl.obolibrary.org/obo/GAZ_00117526">
        <obo:RO_0001025 rdf:resource="http://purl.obolibrary.org/obo/GAZ_00014882"/>
        <obo:RO_0001025 rdf:resource="http://purl.obolibrary.org/obo/GAZ_00057467"/>
        <obo:IAO_0000115>A region of the Gobi Desert in Mongolia, in which important fossil finds have been made.</obo:IAO_0000115>
        <oboInOwl:hasOBONamespace>GAZ</oboInOwl:hasOBONamespace>
        <oboInOwl:id>GAZ:00117526</oboInOwl:id>
        <rdfs:label>Flaming Cliffs</rdfs:label>
    </owl:NamedIndividual>
    


    <!-- http://purl.obolibrary.org/obo/GAZ_00117527 -->

    <owl:NamedIndividual rdf:about="http://purl.obolibrary.org/obo/GAZ_00117527">
        <obo:RO_0001025 rdf:resource="http://purl.obolibrary.org/obo/GAZ_00014885"/>
        <obo:IAO_0000115>A large valley in northwestern Khovsgol Aimag, Mongolia. It is situated between the Ulaan Taiga and Khoridol Saridag ranges at an altitude of about 1600 m, about 160 km long and 40 km wide.</obo:IAO_0000115>
        <oboInOwl:hasOBONamespace>GAZ</oboInOwl:hasOBONamespace>
        <oboInOwl:id>GAZ:00117527</oboInOwl:id>
        <rdfs:label>Darkhad Valley</rdfs:label>
    </owl:NamedIndividual>
    


    <!-- http://purl.obolibrary.org/obo/GAZ_00117528 -->

    <owl:NamedIndividual rdf:about="http://purl.obolibrary.org/obo/GAZ_00117528">
        <obo:RO_0001025 rdf:resource="http://purl.obolibrary.org/obo/GAZ_00014878"/>
        <obo:IAO_0000115>A freshwater (?) lake S of Olgii.</obo:IAO_0000115>
        <oboInOwl:hasOBONamespace>GAZ</oboInOwl:hasOBONamespace>
        <oboInOwl:id>GAZ:00117528</oboInOwl:id>
        <rdfs:label>Tolbo Nuur</rdfs:label>
    </owl:NamedIndividual>
    


    <!-- http://purl.obolibrary.org/obo/GAZ_00117529 -->

    <owl:NamedIndividual rdf:about="http://purl.obolibrary.org/obo/GAZ_00117529">
        <obo:RO_0001025 rdf:resource="http://purl.obolibrary.org/obo/GAZ_00014878"/>
        <obo:IAO_0000115>A national park.</obo:IAO_0000115>
        <oboInOwl:hasOBONamespace>GAZ</oboInOwl:hasOBONamespace>
        <oboInOwl:id>GAZ:00117529</oboInOwl:id>
        <rdfs:label>Siilkhemiin Nuruu National Park</rdfs:label>
    </owl:NamedIndividual>
    


    <!-- http://purl.obolibrary.org/obo/GAZ_00117530 -->

    <owl:NamedIndividual rdf:about="http://purl.obolibrary.org/obo/GAZ_00117530">
        <obo:RO_0001025 rdf:resource="http://purl.obolibrary.org/obo/GAZ_00014878"/>
        <obo:IAO_0000115>A protected area.</obo:IAO_0000115>
        <oboInOwl:hasOBONamespace>GAZ</oboInOwl:hasOBONamespace>
        <oboInOwl:id>GAZ:00117530</oboInOwl:id>
        <rdfs:label>Khokh Serkhiin Nuruu Protected Area</rdfs:label>
    </owl:NamedIndividual>
    


    <!-- http://purl.obolibrary.org/obo/GAZ_00117531 -->

    <owl:NamedIndividual rdf:about="http://purl.obolibrary.org/obo/GAZ_00117531">
        <obo:RO_0001025 rdf:resource="http://purl.obolibrary.org/obo/GAZ_00014878"/>
        <obo:IAO_0000115>A protected area.</obo:IAO_0000115>
        <oboInOwl:hasOBONamespace>GAZ</oboInOwl:hasOBONamespace>
        <oboInOwl:id>GAZ:00117531</oboInOwl:id>
        <rdfs:label>Develiin Aral Natural Reserve</rdfs:label>
    </owl:NamedIndividual>
    


    <!-- http://purl.obolibrary.org/obo/GAZ_00117532 -->

    <owl:NamedIndividual rdf:about="http://purl.obolibrary.org/obo/GAZ_00117532">
        <obo:RO_0001025 rdf:resource="http://purl.obolibrary.org/obo/GAZ_00117531"/>
        <obo:IAO_0000115>An island at the confluence of the rivers Lsan Khooloi and Khovd.</obo:IAO_0000115>
        <oboInOwl:hasOBONamespace>GAZ</oboInOwl:hasOBONamespace>
        <oboInOwl:id>GAZ:00117532</oboInOwl:id>
        <rdfs:label>Develiin Island</rdfs:label>
    </owl:NamedIndividual>
    


    <!-- http://purl.obolibrary.org/obo/GAZ_00117533 -->

    <owl:NamedIndividual rdf:about="http://purl.obolibrary.org/obo/GAZ_00117533">
        <obo:RO_0001025 rdf:resource="http://purl.obolibrary.org/obo/GAZ_00027141"/>
        <obo:IAO_0000115>The fourth-largest city in Mongolia. It is the capital of the aimag (province) of Dornod and city administrative unit official name is Kherlen sum. It is situated at the Kherlen River, at an elevation of 747 m above sea.</obo:IAO_0000115>
        <oboInOwl:hasOBONamespace>GAZ</oboInOwl:hasOBONamespace>
        <oboInOwl:id>GAZ:00117533</oboInOwl:id>
        <rdfs:label>Choibalsan City</rdfs:label>
    </owl:NamedIndividual>
    


    <!-- http://purl.obolibrary.org/obo/GAZ_00117534 -->

    <owl:NamedIndividual rdf:about="http://purl.obolibrary.org/obo/GAZ_00117534">
        <obo:RO_0001025 rdf:resource="http://purl.obolibrary.org/obo/GAZ_00027213"/>
        <obo:IAO_0000115>A populated place. A city in Mongolia. It is the capital of Govisumber Province, in the east-central part of the country. Choir is a center of the Sumber sum of Govisumber Province.</obo:IAO_0000115>
        <oboInOwl:hasOBONamespace>GAZ</oboInOwl:hasOBONamespace>
        <oboInOwl:id>GAZ:00117534</oboInOwl:id>
        <rdfs:label>Choir</rdfs:label>
    </owl:NamedIndividual>
    


    <!-- http://purl.obolibrary.org/obo/GAZ_00117535 -->

    <owl:NamedIndividual rdf:about="http://purl.obolibrary.org/obo/GAZ_00117535">
        <obo:RO_0001025 rdf:resource="http://purl.obolibrary.org/obo/GAZ_00014873"/>
        <obo:IAO_0000115>A national park located in the northeast of Khentii Aimag.</obo:IAO_0000115>
        <oboInOwl:hasOBONamespace>GAZ</oboInOwl:hasOBONamespace>
        <oboInOwl:id>GAZ:00117535</oboInOwl:id>
        <rdfs:label>Balj-Onon National Park</rdfs:label>
    </owl:NamedIndividual>
    


    <!-- http://purl.obolibrary.org/obo/GAZ_00117536 -->

    <owl:NamedIndividual rdf:about="http://purl.obolibrary.org/obo/GAZ_00117536">
        <obo:RO_0001025 rdf:resource="http://purl.obolibrary.org/obo/GAZ_00027245"/>
        <obo:IAO_0000115>The capital of the Khovd Province of Mongolia.</obo:IAO_0000115>
        <oboInOwl:hasOBONamespace>GAZ</oboInOwl:hasOBONamespace>
        <oboInOwl:id>GAZ:00117536</oboInOwl:id>
        <rdfs:label>Khovd City</rdfs:label>
    </owl:NamedIndividual>
    


    <!-- http://purl.obolibrary.org/obo/GAZ_00117537 -->

    <owl:NamedIndividual rdf:about="http://purl.obolibrary.org/obo/GAZ_00117537">
        <obo:RO_0001025 rdf:resource="http://purl.obolibrary.org/obo/GAZ_00027245"/>
        <obo:IAO_0000115>A protected area.</obo:IAO_0000115>
        <oboInOwl:hasOBONamespace>GAZ</oboInOwl:hasOBONamespace>
        <oboInOwl:id>GAZ:00117537</oboInOwl:id>
        <rdfs:label>Mankhan Nature Preserve</rdfs:label>
    </owl:NamedIndividual>
    


    <!-- http://purl.obolibrary.org/obo/GAZ_00117538 -->

    <owl:NamedIndividual rdf:about="http://purl.obolibrary.org/obo/GAZ_00117538">
        <rdf:type rdf:resource="http://purl.obolibrary.org/obo/ENVO_00000856"/>
        <obo:RO_0001025 rdf:resource="http://purl.obolibrary.org/obo/GAZ_00027299"/>
        <obo:RO_0001025 rdf:resource="http://purl.obolibrary.org/obo/GAZ_00027324"/>
        <obo:IAO_0000115>A populated place. A town in eastern Mongolia and the capital of Sukhbaatar Province. The town is a sum (district) of Sukhbaatar Province. An enclave in Sukhbaatar Sum.</obo:IAO_0000115>
        <oboInOwl:hasOBONamespace>GAZ</oboInOwl:hasOBONamespace>
        <oboInOwl:id>GAZ:00117538</oboInOwl:id>
        <rdfs:label>Baruun-Urt</rdfs:label>
    </owl:NamedIndividual>
    


    <!-- http://purl.obolibrary.org/obo/GAZ_00117539 -->

    <owl:NamedIndividual rdf:about="http://purl.obolibrary.org/obo/GAZ_00117539">
        <obo:RO_0001025 rdf:resource="http://purl.obolibrary.org/obo/GAZ_00014869"/>
        <obo:IAO_0000115>A protected area. Established 2003.</obo:IAO_0000115>
        <oboInOwl:hasOBONamespace>GAZ</oboInOwl:hasOBONamespace>
        <oboInOwl:id>GAZ:00117539</oboInOwl:id>
        <rdfs:label>Gun-Galuut Nature Reserve</rdfs:label>
    </owl:NamedIndividual>
    


    <!-- http://purl.obolibrary.org/obo/GAZ_00117540 -->

    <owl:NamedIndividual rdf:about="http://purl.obolibrary.org/obo/GAZ_00117540">
        <obo:RO_0001025 rdf:resource="http://purl.obolibrary.org/obo/GAZ_00014876"/>
        <oboInOwl:hasOBONamespace>GAZ</oboInOwl:hasOBONamespace>
        <oboInOwl:id>GAZ:00117540</oboInOwl:id>
        <rdfs:label>Achit Nuur Depression</rdfs:label>
    </owl:NamedIndividual>
    


    <!-- http://purl.obolibrary.org/obo/GAZ_00117541 -->

    <owl:NamedIndividual rdf:about="http://purl.obolibrary.org/obo/GAZ_00117541">
        <obo:RO_0001025 rdf:resource="http://purl.obolibrary.org/obo/GAZ_00027363"/>
        <obo:RO_0001025 rdf:resource="http://purl.obolibrary.org/obo/GAZ_00057910"/>
        <obo:IAO_0000115>A saline lake in western Mongolia, north-west of the Great Lakes Depression, near the western edge of the Uvs Nuur basin.</obo:IAO_0000115>
        <oboInOwl:hasOBONamespace>GAZ</oboInOwl:hasOBONamespace>
        <oboInOwl:id>GAZ:00117541</oboInOwl:id>
        <rdfs:label>Uureg Nuur</rdfs:label>
    </owl:NamedIndividual>
    


    <!-- http://purl.obolibrary.org/obo/GAZ_00117542 -->

    <owl:NamedIndividual rdf:about="http://purl.obolibrary.org/obo/GAZ_00117542">
        <obo:RO_0001025 rdf:resource="http://purl.obolibrary.org/obo/GAZ_00008744"/>
        <obo:IAO_0000115>An independent municipality not part of any Province of Mongolia.</obo:IAO_0000115>
        <oboInOwl:hasOBONamespace>GAZ</oboInOwl:hasOBONamespace>
        <oboInOwl:id>GAZ:00117542</oboInOwl:id>
        <rdfs:label>Municipality of Ulan Bator</rdfs:label>
    </owl:NamedIndividual>
    


    <!-- http://purl.obolibrary.org/obo/GAZ_00117543 -->

    <owl:NamedIndividual rdf:about="http://purl.obolibrary.org/obo/GAZ_00117543">
        <obo:RO_0001025 rdf:resource="http://purl.obolibrary.org/obo/GAZ_00117542"/>
        <obo:IAO_0000115>The capital and largest city of Mongolia.</obo:IAO_0000115>
        <oboInOwl:hasOBONamespace>GAZ</oboInOwl:hasOBONamespace>
        <oboInOwl:id>GAZ:00117543</oboInOwl:id>
        <rdfs:label>Ulan Bator</rdfs:label>
    </owl:NamedIndividual>
    


    <!-- http://purl.obolibrary.org/obo/GAZ_00117544 -->

    <owl:NamedIndividual rdf:about="http://purl.obolibrary.org/obo/GAZ_00117544">
        <obo:RO_0001025 rdf:resource="http://purl.obolibrary.org/obo/GAZ_00117543"/>
        <obo:IAO_0000115>One of nine duuregs (districts) of the Mongolian capital of Ulan Bator. Baganuur is actually a separate city, located as an exclave of 620 km2 at the border between the Tov and Khentii aimags.</obo:IAO_0000115>
        <oboInOwl:hasOBONamespace>GAZ</oboInOwl:hasOBONamespace>
        <oboInOwl:id>GAZ:00117544</oboInOwl:id>
        <rdfs:label>Baganuur District</rdfs:label>
    </owl:NamedIndividual>
    


    <!-- http://purl.obolibrary.org/obo/GAZ_00117545 -->

    <owl:NamedIndividual rdf:about="http://purl.obolibrary.org/obo/GAZ_00117545">
        <obo:RO_0001025 rdf:resource="http://purl.obolibrary.org/obo/GAZ_00117543"/>
        <obo:IAO_0000115>One of nine duuregs (districts) of the Mongolian capital of Ulan Bator.</obo:IAO_0000115>
        <oboInOwl:hasOBONamespace>GAZ</oboInOwl:hasOBONamespace>
        <oboInOwl:id>GAZ:00117545</oboInOwl:id>
        <rdfs:label>Khan Uul District</rdfs:label>
    </owl:NamedIndividual>
    


    <!-- http://purl.obolibrary.org/obo/GAZ_00117546 -->

    <owl:NamedIndividual rdf:about="http://purl.obolibrary.org/obo/GAZ_00117546">
        <obo:RO_0001025 rdf:resource="http://purl.obolibrary.org/obo/GAZ_00117543"/>
        <obo:IAO_0000115>One of nine duuregs (districts) of the Mongolian capital of Ulan Bator.</obo:IAO_0000115>
        <oboInOwl:hasOBONamespace>GAZ</oboInOwl:hasOBONamespace>
        <oboInOwl:id>GAZ:00117546</oboInOwl:id>
        <rdfs:label>Sukhbaatar District</rdfs:label>
    </owl:NamedIndividual>
    


    <!-- http://purl.obolibrary.org/obo/GAZ_00117547 -->

    <owl:NamedIndividual rdf:about="http://purl.obolibrary.org/obo/GAZ_00117547">
        <obo:RO_0001025 rdf:resource="http://purl.obolibrary.org/obo/GAZ_00117543"/>
        <obo:IAO_0000115>One of nine duuregs (districts) of the Mongolian capital of Ulan Bator. Bagakhangai is an exclave of 140 km2 in Tov Province, southeast of the capital.</obo:IAO_0000115>
        <oboInOwl:hasOBONamespace>GAZ</oboInOwl:hasOBONamespace>
        <oboInOwl:id>GAZ:00117547</oboInOwl:id>
        <rdfs:label>Bagakhangai District</rdfs:label>
    </owl:NamedIndividual>
    


    <!-- http://purl.obolibrary.org/obo/GAZ_00117548 -->

    <owl:NamedIndividual rdf:about="http://purl.obolibrary.org/obo/GAZ_00117548">
        <obo:RO_0001025 rdf:resource="http://purl.obolibrary.org/obo/GAZ_00117543"/>
        <obo:IAO_0000115>One of nine duuregs (districts) of the Mongolian capital of Ulan Bator.</obo:IAO_0000115>
        <oboInOwl:hasOBONamespace>GAZ</oboInOwl:hasOBONamespace>
        <oboInOwl:id>GAZ:00117548</oboInOwl:id>
        <rdfs:label>Chingeltei District</rdfs:label>
    </owl:NamedIndividual>
    


    <!-- http://purl.obolibrary.org/obo/GAZ_00117549 -->

    <owl:NamedIndividual rdf:about="http://purl.obolibrary.org/obo/GAZ_00117549">
        <obo:RO_0001025 rdf:resource="http://purl.obolibrary.org/obo/GAZ_00117543"/>
        <obo:IAO_0000115>One of nine duuregs (districts) of the Mongolian capital of Ulan Bator.</obo:IAO_0000115>
        <oboInOwl:hasOBONamespace>GAZ</oboInOwl:hasOBONamespace>
        <oboInOwl:id>GAZ:00117549</oboInOwl:id>
        <rdfs:label>Bayanzurkh District</rdfs:label>
    </owl:NamedIndividual>
    


    <!-- http://purl.obolibrary.org/obo/GAZ_00117550 -->

    <owl:NamedIndividual rdf:about="http://purl.obolibrary.org/obo/GAZ_00117550">
        <obo:RO_0001025 rdf:resource="http://purl.obolibrary.org/obo/GAZ_00117543"/>
        <obo:IAO_0000115>One of nine duuregs (districts) of the Mongolian capital of Ulan Bator.</obo:IAO_0000115>
        <oboInOwl:hasOBONamespace>GAZ</oboInOwl:hasOBONamespace>
        <oboInOwl:id>GAZ:00117550</oboInOwl:id>
        <rdfs:label>Songino Khairkhan District</rdfs:label>
    </owl:NamedIndividual>
    


    <!-- http://purl.obolibrary.org/obo/GAZ_00117551 -->

    <owl:NamedIndividual rdf:about="http://purl.obolibrary.org/obo/GAZ_00117551">
        <obo:RO_0001025 rdf:resource="http://purl.obolibrary.org/obo/GAZ_00117543"/>
        <obo:IAO_0000115>One of nine duuregs (districts) of the Mongolian capital of Ulan Bator.</obo:IAO_0000115>
        <oboInOwl:hasOBONamespace>GAZ</oboInOwl:hasOBONamespace>
        <oboInOwl:id>GAZ:00117551</oboInOwl:id>
        <rdfs:label>Bayangol District</rdfs:label>
    </owl:NamedIndividual>
    


    <!-- http://purl.obolibrary.org/obo/GAZ_00117552 -->

    <owl:NamedIndividual rdf:about="http://purl.obolibrary.org/obo/GAZ_00117552">
        <obo:RO_0001025 rdf:resource="http://purl.obolibrary.org/obo/GAZ_00117543"/>
        <obo:IAO_0000115>One of nine duuregs (districts) of the Mongolian capital of Ulan Bator.</obo:IAO_0000115>
        <oboInOwl:hasOBONamespace>GAZ</oboInOwl:hasOBONamespace>
        <oboInOwl:id>GAZ:00117552</oboInOwl:id>
        <rdfs:label>Nalaikh District</rdfs:label>
    </owl:NamedIndividual>
    


    <!-- http://purl.obolibrary.org/obo/GAZ_00150545 -->

    <owl:NamedIndividual rdf:about="http://purl.obolibrary.org/obo/GAZ_00150545">
        <obo:IAO_0000115>A World Herritage Site consisting of the Altai and Katun Natural Reserves, Lake Teletskoye, Belukha Mountain, and the Ukok Plateau.</obo:IAO_0000115>
        <oboInOwl:hasOBONamespace>GAZ</oboInOwl:hasOBONamespace>
        <oboInOwl:id>GAZ:00150545</oboInOwl:id>
        <rdfs:label>Golden Mountains of Altai</rdfs:label>
    </owl:NamedIndividual>
    


    <!-- http://purl.obolibrary.org/obo/GAZ_00150546 -->

    <owl:NamedIndividual rdf:about="http://purl.obolibrary.org/obo/GAZ_00150546">
        <obo:RO_0001025 rdf:resource="http://purl.obolibrary.org/obo/GAZ_00150545"/>
        <obo:IAO_0000115>A remote and pristine grasslands area located in the heart of southwestern Siberia, the Altai Mountains region of Russia near the borders with China, Kazakhstan and Mongolia.</obo:IAO_0000115>
        <oboInOwl:hasOBONamespace>GAZ</oboInOwl:hasOBONamespace>
        <oboInOwl:id>GAZ:00150546</oboInOwl:id>
        <rdfs:label>Ukok Plateau</rdfs:label>
    </owl:NamedIndividual>
    


    <!-- http://purl.obolibrary.org/obo/GAZ_00150547 -->

    <owl:NamedIndividual rdf:about="http://purl.obolibrary.org/obo/GAZ_00150547">
        <obo:RO_0001025 rdf:resource="http://purl.obolibrary.org/obo/GAZ_00150545"/>
        <obo:IAO_0000115>A protected area (zapovednik).</obo:IAO_0000115>
        <oboInOwl:hasOBONamespace>GAZ</oboInOwl:hasOBONamespace>
        <oboInOwl:id>GAZ:00150547</oboInOwl:id>
        <rdfs:label>Altai Natural Reserve</rdfs:label>
    </owl:NamedIndividual>
    


    <!-- http://purl.obolibrary.org/obo/GAZ_00150548 -->

    <owl:NamedIndividual rdf:about="http://purl.obolibrary.org/obo/GAZ_00150548">
        <obo:RO_0001025 rdf:resource="http://purl.obolibrary.org/obo/GAZ_00150545"/>
        <obo:IAO_0000115>A protected area (zapovednik). Includes the upper Katun River in the Altay Mountains.</obo:IAO_0000115>
        <oboInOwl:hasOBONamespace>GAZ</oboInOwl:hasOBONamespace>
        <oboInOwl:id>GAZ:00150548</oboInOwl:id>
        <rdfs:label>Katun Natural Reserve</rdfs:label>
    </owl:NamedIndividual>
    


    <!-- http://purl.obolibrary.org/obo/GAZ_00247573 -->

    <owl:NamedIndividual rdf:about="http://purl.obolibrary.org/obo/GAZ_00247573">
        <obo:RO_0001025 rdf:resource="http://purl.obolibrary.org/obo/GAZ_00114665"/>
        <obo:IAO_0000115>A large saline lake with associated brackish marshes and meadows, at the extreme western end of the Junggar Basin.</obo:IAO_0000115>
        <oboInOwl:hasOBONamespace>GAZ</oboInOwl:hasOBONamespace>
        <oboInOwl:id>GAZ:00247573</oboInOwl:id>
        <rdfs:label>Ebinur Hu</rdfs:label>
    </owl:NamedIndividual>
    


    <!-- http://purl.obolibrary.org/obo/GAZ_00247579 -->

    <owl:NamedIndividual rdf:about="http://purl.obolibrary.org/obo/GAZ_00247579">
        <obo:IAO_0000115>A large freshwater lake, about 23 km long and three km wide, and associated marshes in the northern Altai Mountains. The lake is fed by two small rivers rising in the Youyi Feng Huten Orgil mountains on the Russian and Mongolian borders (peaks to 4,374 m), and drains southeast into a small tributary of the Ertix He (Irtysh River).</obo:IAO_0000115>
        <oboInOwl:hasOBONamespace>GAZ</oboInOwl:hasOBONamespace>
        <oboInOwl:id>GAZ:00247579</oboInOwl:id>
        <rdfs:label>Chianassu Hu</rdfs:label>
    </owl:NamedIndividual>
    


    <!-- http://purl.obolibrary.org/obo/GAZ_00247581 -->

    <owl:NamedIndividual rdf:about="http://purl.obolibrary.org/obo/GAZ_00247581">
        <obo:IAO_0000115>Five small freshwater lakes, each 150-350 ha in extent, many smaller ponds, freshwater marshes, mountain bogs, and fast-flowing mountain streams at the headwaters of the Ulungur He in the southern Altai Shan mountains. Located Qinghe County, in the southern Altai Mountains on the Mongolian border, 420 km northeast of Wulumqi (Urumqi), Xinjiang Zizhiqu.</obo:IAO_0000115>
        <oboInOwl:hasOBONamespace>GAZ</oboInOwl:hasOBONamespace>
        <oboInOwl:id>GAZ:00247581</oboInOwl:id>
        <rdfs:label>Southern Altai Lakes</rdfs:label>
    </owl:NamedIndividual>
    


    <!-- http://purl.obolibrary.org/obo/GAZ_00252209 -->

    <owl:NamedIndividual rdf:about="http://purl.obolibrary.org/obo/GAZ_00252209"/>
    


    <!-- http://purl.obolibrary.org/obo/GAZ_00252217 -->

    <owl:NamedIndividual rdf:about="http://purl.obolibrary.org/obo/GAZ_00252217">
        <obo:RO_0001025 rdf:resource="http://purl.obolibrary.org/obo/GAZ_00014880"/>
        <obo:IAO_0000115>A river in Arkhangai. It springs from the Terkhiin Tsagaan Nuur and is a tributary of the Chuluut River.</obo:IAO_0000115>
        <oboInOwl:hasOBONamespace>GAZ</oboInOwl:hasOBONamespace>
        <oboInOwl:id>GAZ:00252217</oboInOwl:id>
        <rdfs:label>Suman River</rdfs:label>
    </owl:NamedIndividual>
    


    <!-- http://purl.obolibrary.org/obo/GAZ_00252218 -->

    <owl:NamedIndividual rdf:about="http://purl.obolibrary.org/obo/GAZ_00252218">
        <obo:RO_0001025 rdf:resource="http://purl.obolibrary.org/obo/GAZ_00014885"/>
        <obo:RO_0001025 rdf:resource="http://purl.obolibrary.org/obo/GAZ_00252209"/>
        <obo:IAO_0000115>A river in the Khovsgol Province in northern Mongolia. Together with the Ider River it is one of the sources of the Selenge River. The source is in the Ulaan Taiga range close to the Russian border, the confluence with the Ider River is in Tomorbulag sum.</obo:IAO_0000115>
        <oboInOwl:hasOBONamespace>GAZ</oboInOwl:hasOBONamespace>
        <oboInOwl:id>GAZ:00252218</oboInOwl:id>
        <rdfs:label>Delgermoron</rdfs:label>
    </owl:NamedIndividual>
    


    <!-- http://purl.obolibrary.org/obo/GAZ_00252225 -->

    <owl:NamedIndividual rdf:about="http://purl.obolibrary.org/obo/GAZ_00252225">
        <obo:IAO_0000115>A river in the Buryat Republic, Russia. It is a right tributary of the Selenga, which it meets near the city Ulan-Ude.</obo:IAO_0000115>
        <oboInOwl:hasOBONamespace>GAZ</oboInOwl:hasOBONamespace>
        <oboInOwl:id>GAZ:00252225</oboInOwl:id>
        <rdfs:label>Uda River</rdfs:label>
    </owl:NamedIndividual>
    


    <!-- http://purl.obolibrary.org/obo/GAZ_00252236 -->

    <owl:NamedIndividual rdf:about="http://purl.obolibrary.org/obo/GAZ_00252236">
        <rdf:type rdf:resource="http://purl.obolibrary.org/obo/ENVO_00000106"/>
        <obo:IAO_0000115>A range in the E Khentii Mountains.</obo:IAO_0000115>
        <oboInOwl:hasOBONamespace>GAZ</oboInOwl:hasOBONamespace>
        <oboInOwl:id>GAZ:00252236</oboInOwl:id>
        <rdfs:label>Hentiyn Nuruu Mountains</rdfs:label>
    </owl:NamedIndividual>
    


    <!-- http://purl.obolibrary.org/obo/GAZ_00252243 -->

    <owl:NamedIndividual rdf:about="http://purl.obolibrary.org/obo/GAZ_00252243">
        <obo:RO_0001025 rdf:resource="http://purl.obolibrary.org/obo/GAZ_00027286"/>
        <obo:IAO_0000115>A populated place. A city. Kharkhorin is located at the lower end of the upper valley of the Orkhon River, part of the World Heritage Site Orkhon Valley Cultural Landscape. The location marks the eastern foothills of the Khangai Mountains, where they meet the rolling steppe of central Mongolia.</obo:IAO_0000115>
        <oboInOwl:hasOBONamespace>GAZ</oboInOwl:hasOBONamespace>
        <oboInOwl:id>GAZ:00252243</oboInOwl:id>
        <rdfs:label>Kharkhorin</rdfs:label>
    </owl:NamedIndividual>
    


    <!-- http://purl.obolibrary.org/obo/GAZ_00252244 -->

    <owl:NamedIndividual rdf:about="http://purl.obolibrary.org/obo/GAZ_00252244">
        <obo:RO_0001025 rdf:resource="http://purl.obolibrary.org/obo/GAZ_00014880"/>
        <obo:RO_0001025 rdf:resource="http://purl.obolibrary.org/obo/GAZ_00057876"/>
        <obo:IAO_0000115>A river flowing through the valleys of the Khangai Mountains in central Mongolia. It is a main tributary of the Orkhon River.</obo:IAO_0000115>
        <oboInOwl:hasOBONamespace>GAZ</oboInOwl:hasOBONamespace>
        <oboInOwl:id>GAZ:00252244</oboInOwl:id>
        <rdfs:label>Tamir River</rdfs:label>
    </owl:NamedIndividual>
    


    <!-- http://purl.obolibrary.org/obo/GAZ_00252245 -->

    <owl:NamedIndividual rdf:about="http://purl.obolibrary.org/obo/GAZ_00252245">
        <obo:RO_0001025 rdf:resource="http://purl.obolibrary.org/obo/GAZ_00026102"/>
        <obo:RO_0001025 rdf:resource="http://purl.obolibrary.org/obo/GAZ_00054873"/>
        <obo:IAO_0000115>An archeological site.</obo:IAO_0000115>
        <oboInOwl:hasOBONamespace>GAZ</oboInOwl:hasOBONamespace>
        <oboInOwl:id>GAZ:00252245</oboInOwl:id>
        <rdfs:label>Kharabalghasun</rdfs:label>
    </owl:NamedIndividual>
    


    <!-- http://purl.obolibrary.org/obo/GAZ_00252246 -->

    <owl:NamedIndividual rdf:about="http://purl.obolibrary.org/obo/GAZ_00252246">
        <obo:RO_0001025 rdf:resource="http://purl.obolibrary.org/obo/GAZ_00014886"/>
        <obo:RO_0001025 rdf:resource="http://purl.obolibrary.org/obo/GAZ_00054873"/>
        <obo:IAO_0000115>An archeological site.</obo:IAO_0000115>
        <oboInOwl:hasOBONamespace>GAZ</oboInOwl:hasOBONamespace>
        <oboInOwl:id>GAZ:00252246</oboInOwl:id>
        <rdfs:label>Karakorum</rdfs:label>
    </owl:NamedIndividual>
    


    <!-- http://purl.obolibrary.org/obo/GAZ_00252247 -->

    <owl:NamedIndividual rdf:about="http://purl.obolibrary.org/obo/GAZ_00252247">
        <obo:RO_0001025 rdf:resource="http://purl.obolibrary.org/obo/GAZ_00014878"/>
        <obo:IAO_0000115>Three lakes situated in an elongated basin 50-60 km in length at the foot of the Tavan Bogd Uul mountain.</obo:IAO_0000115>
        <oboInOwl:hasOBONamespace>GAZ</oboInOwl:hasOBONamespace>
        <oboInOwl:id>GAZ:00252247</oboInOwl:id>
        <rdfs:label>Kobdossk Lakes</rdfs:label>
    </owl:NamedIndividual>
    


    <!-- http://purl.obolibrary.org/obo/GAZ_00252248 -->

    <owl:NamedIndividual rdf:about="http://purl.obolibrary.org/obo/GAZ_00252248">
        <obo:RO_0001025 rdf:resource="http://purl.obolibrary.org/obo/GAZ_00252247"/>
        <obo:IAO_0000115>A sub-alpine freshwater lake.</obo:IAO_0000115>
        <oboInOwl:hasOBONamespace>GAZ</oboInOwl:hasOBONamespace>
        <oboInOwl:id>GAZ:00252248</oboInOwl:id>
        <rdfs:label>Hoton Nuur</rdfs:label>
    </owl:NamedIndividual>
    


    <!-- http://purl.obolibrary.org/obo/GAZ_00252249 -->

    <owl:NamedIndividual rdf:about="http://purl.obolibrary.org/obo/GAZ_00252249">
        <obo:RO_0001025 rdf:resource="http://purl.obolibrary.org/obo/GAZ_00252247"/>
        <obo:IAO_0000115>A sub-alpine freshwater lake.</obo:IAO_0000115>
        <oboInOwl:hasOBONamespace>GAZ</oboInOwl:hasOBONamespace>
        <oboInOwl:id>GAZ:00252249</oboInOwl:id>
        <rdfs:label>Orgon Nuur</rdfs:label>
    </owl:NamedIndividual>
    


    <!-- http://purl.obolibrary.org/obo/GAZ_00252250 -->

    <owl:NamedIndividual rdf:about="http://purl.obolibrary.org/obo/GAZ_00252250">
        <obo:RO_0001025 rdf:resource="http://purl.obolibrary.org/obo/GAZ_00252247"/>
        <obo:IAO_0000115>A sub-alpine freshwater lake.</obo:IAO_0000115>
        <oboInOwl:hasOBONamespace>GAZ</oboInOwl:hasOBONamespace>
        <oboInOwl:id>GAZ:00252250</oboInOwl:id>
        <rdfs:label>Dayan Nuur</rdfs:label>
    </owl:NamedIndividual>
    


    <!-- http://purl.obolibrary.org/obo/GAZ_00252251 -->

    <owl:NamedIndividual rdf:about="http://purl.obolibrary.org/obo/GAZ_00252251">
        <obo:RO_0001025 rdf:resource="http://purl.obolibrary.org/obo/GAZ_00252247"/>
        <obo:IAO_0000115>A freshwater lake. Located in an elongated basin in the Altai Mountain region of the Central Asian Internal Drainage Basin, near the Chinese border, 110 km WSW of Olgiy, Bayan-Olgiy Province.</obo:IAO_0000115>
        <oboInOwl:hasOBONamespace>GAZ</oboInOwl:hasOBONamespace>
        <oboInOwl:id>GAZ:00252251</oboInOwl:id>
        <rdfs:label>Horgon Nuur</rdfs:label>
    </owl:NamedIndividual>
    


    <!-- http://purl.obolibrary.org/obo/GAZ_00252261 -->

    <owl:NamedIndividual rdf:about="http://purl.obolibrary.org/obo/GAZ_00252261">
        <obo:RO_0001025 rdf:resource="http://purl.obolibrary.org/obo/GAZ_00014878"/>
        <obo:IAO_0000115>A freshwater lake. Located in a basin close to the Russian border, about 60-65 km southwest of Orog Nuur. It receives inflow from the Hatugiyn, Buh Moron and Ulyastayn rivers in the northwest; the ouflow in the southeast forms the Usan Holoy River.</obo:IAO_0000115>
        <oboInOwl:hasOBONamespace>GAZ</oboInOwl:hasOBONamespace>
        <oboInOwl:id>GAZ:00252261</oboInOwl:id>
        <rdfs:label>Achit Nuur</rdfs:label>
    </owl:NamedIndividual>
    


    <!-- http://purl.obolibrary.org/obo/GAZ_00252265 -->

    <owl:NamedIndividual rdf:about="http://purl.obolibrary.org/obo/GAZ_00252265">
        <obo:RO_0001025 rdf:resource="http://purl.obolibrary.org/obo/GAZ_00014878"/>
        <obo:IAO_0000115>A slightly saline lake. Located in a basin in the Altai Mountains close to the Russian border, 70 km WNW of Ulaangom, Bayan-Olgiy Province.</obo:IAO_0000115>
        <oboInOwl:hasOBONamespace>GAZ</oboInOwl:hasOBONamespace>
        <oboInOwl:id>GAZ:00252265</oboInOwl:id>
        <rdfs:label>Orog Nuur</rdfs:label>
    </owl:NamedIndividual>
    


    <!-- http://purl.obolibrary.org/obo/GAZ_00252270 -->

    <owl:NamedIndividual rdf:about="http://purl.obolibrary.org/obo/GAZ_00252270">
        <obo:IAO_0000115>A river between Khar Nuur and Khar-Us Nuur.</obo:IAO_0000115>
        <oboInOwl:hasOBONamespace>GAZ</oboInOwl:hasOBONamespace>
        <oboInOwl:id>GAZ:00252270</oboInOwl:id>
        <rdfs:label>Conoharayh Gol</rdfs:label>
    </owl:NamedIndividual>
    


    <!-- http://purl.obolibrary.org/obo/GAZ_00252271 -->

    <owl:NamedIndividual rdf:about="http://purl.obolibrary.org/obo/GAZ_00252271">
        <obo:IAO_0000115>A river connecting Khar Nuur and Dorgon Nuur.</obo:IAO_0000115>
        <oboInOwl:hasOBONamespace>GAZ</oboInOwl:hasOBONamespace>
        <oboInOwl:id>GAZ:00252271</oboInOwl:id>
        <rdfs:label>Homin Holoy River</rdfs:label>
    </owl:NamedIndividual>
    


    <!-- http://purl.obolibrary.org/obo/GAZ_00252272 -->

    <owl:NamedIndividual rdf:about="http://purl.obolibrary.org/obo/GAZ_00252272">
        <obo:RO_0001025 rdf:resource="http://purl.obolibrary.org/obo/GAZ_00008744"/>
        <obo:IAO_0000115>A freshwater endorheic lake. Located at the western edge of the Khangayn Plateau overlooking the Great Lakes Depression, 90 km southwest of Telmen Nuur.</obo:IAO_0000115>
        <oboInOwl:hasOBONamespace>GAZ</oboInOwl:hasOBONamespace>
        <oboInOwl:id>GAZ:00252272</oboInOwl:id>
        <rdfs:label>Hunguyn Har Nuur</rdfs:label>
    </owl:NamedIndividual>
    


    <!-- http://purl.obolibrary.org/obo/GAZ_00252273 -->

    <owl:NamedIndividual rdf:about="http://purl.obolibrary.org/obo/GAZ_00252273">
        <obo:RO_0001025 rdf:resource="http://purl.obolibrary.org/obo/GAZ_00252276"/>
        <obo:IAO_0000115>A river.</obo:IAO_0000115>
        <oboInOwl:hasOBONamespace>GAZ</oboInOwl:hasOBONamespace>
        <oboInOwl:id>GAZ:00252273</oboInOwl:id>
        <rdfs:label>Muhar Hunguyn Gol</rdfs:label>
    </owl:NamedIndividual>
    


    <!-- http://purl.obolibrary.org/obo/GAZ_00252274 -->

    <owl:NamedIndividual rdf:about="http://purl.obolibrary.org/obo/GAZ_00252274">
        <obo:RO_0001025 rdf:resource="http://purl.obolibrary.org/obo/GAZ_00014877"/>
        <obo:RO_0001025 rdf:resource="http://purl.obolibrary.org/obo/GAZ_00252276"/>
        <obo:IAO_0000115>An endorheic saline lake. Located in the Khangayn Plateau region of the Central Asian Internal Drainage Basin, 215 km WSW of Moron.</obo:IAO_0000115>
        <oboInOwl:hasOBONamespace>GAZ</oboInOwl:hasOBONamespace>
        <oboInOwl:id>GAZ:00252274</oboInOwl:id>
        <rdfs:label>Telmen Nuur</rdfs:label>
    </owl:NamedIndividual>
    


    <!-- http://purl.obolibrary.org/obo/GAZ_00252276 -->

    <owl:NamedIndividual rdf:about="http://purl.obolibrary.org/obo/GAZ_00252276">
        <obo:RO_0001025 rdf:resource="http://purl.obolibrary.org/obo/GAZ_00008744"/>
        <oboInOwl:hasOBONamespace>GAZ</oboInOwl:hasOBONamespace>
        <oboInOwl:id>GAZ:00252276</oboInOwl:id>
        <rdfs:label>Khangayn Plateau</rdfs:label>
    </owl:NamedIndividual>
    


    <!-- http://purl.obolibrary.org/obo/GAZ_00252278 -->

    <owl:NamedIndividual rdf:about="http://purl.obolibrary.org/obo/GAZ_00252278">
        <obo:RO_0001025 rdf:resource="http://purl.obolibrary.org/obo/GAZ_00014885"/>
        <obo:IAO_0000115>A slightly saline lake. Located in the Hangayn Plateau region of the Central Asian Internal Drainage Basin, 90 km SW of Moron, Khovsgol Province.</obo:IAO_0000115>
        <oboInOwl:hasOBONamespace>GAZ</oboInOwl:hasOBONamespace>
        <oboInOwl:id>GAZ:00252278</oboInOwl:id>
        <rdfs:label>Sangiyn Dalay Nuur</rdfs:label>
    </owl:NamedIndividual>
    


    <!-- http://purl.obolibrary.org/obo/GAZ_00252279 -->

    <owl:NamedIndividual rdf:about="http://purl.obolibrary.org/obo/GAZ_00252279">
        <obo:RO_0001025 rdf:resource="http://purl.obolibrary.org/obo/GAZ_00117527"/>
        <obo:IAO_0000115>A lake.</obo:IAO_0000115>
        <oboInOwl:hasOBONamespace>GAZ</oboInOwl:hasOBONamespace>
        <oboInOwl:id>GAZ:00252279</oboInOwl:id>
        <rdfs:label>Targan Nuur</rdfs:label>
    </owl:NamedIndividual>
    


    <!-- http://purl.obolibrary.org/obo/GAZ_00252280 -->

    <owl:NamedIndividual rdf:about="http://purl.obolibrary.org/obo/GAZ_00252280">
        <obo:RO_0001025 rdf:resource="http://purl.obolibrary.org/obo/GAZ_00117527"/>
        <obo:IAO_0000115>A lake.</obo:IAO_0000115>
        <oboInOwl:hasOBONamespace>GAZ</oboInOwl:hasOBONamespace>
        <oboInOwl:id>GAZ:00252280</oboInOwl:id>
        <rdfs:label>Togrog Nuur</rdfs:label>
    </owl:NamedIndividual>
    


    <!-- http://purl.obolibrary.org/obo/GAZ_00252281 -->

    <owl:NamedIndividual rdf:about="http://purl.obolibrary.org/obo/GAZ_00252281">
        <obo:RO_0001025 rdf:resource="http://purl.obolibrary.org/obo/GAZ_00117527"/>
        <obo:IAO_0000115>A lake.</obo:IAO_0000115>
        <oboInOwl:hasOBONamespace>GAZ</oboInOwl:hasOBONamespace>
        <oboInOwl:id>GAZ:00252281</oboInOwl:id>
        <rdfs:label>Sayrt Nuur</rdfs:label>
    </owl:NamedIndividual>
    


    <!-- http://purl.obolibrary.org/obo/GAZ_00252282 -->

    <owl:NamedIndividual rdf:about="http://purl.obolibrary.org/obo/GAZ_00252282">
        <obo:RO_0001025 rdf:resource="http://purl.obolibrary.org/obo/GAZ_00117527"/>
        <obo:IAO_0000115>A lake.</obo:IAO_0000115>
        <oboInOwl:hasOBONamespace>GAZ</oboInOwl:hasOBONamespace>
        <oboInOwl:id>GAZ:00252282</oboInOwl:id>
        <rdfs:label>Duren Nuur</rdfs:label>
    </owl:NamedIndividual>
    


    <!-- http://purl.obolibrary.org/obo/GAZ_00252283 -->

    <owl:NamedIndividual rdf:about="http://purl.obolibrary.org/obo/GAZ_00252283">
        <obo:RO_0001025 rdf:resource="http://purl.obolibrary.org/obo/GAZ_00117527"/>
        <obo:IAO_0000115>A lake.</obo:IAO_0000115>
        <oboInOwl:hasOBONamespace>GAZ</oboInOwl:hasOBONamespace>
        <oboInOwl:id>GAZ:00252283</oboInOwl:id>
        <rdfs:label>Tseutson Nuur</rdfs:label>
    </owl:NamedIndividual>
    


    <!-- http://purl.obolibrary.org/obo/GAZ_00252284 -->

    <owl:NamedIndividual rdf:about="http://purl.obolibrary.org/obo/GAZ_00252284">
        <obo:RO_0001025 rdf:resource="http://purl.obolibrary.org/obo/GAZ_00117527"/>
        <obo:IAO_0000115>A lake.</obo:IAO_0000115>
        <oboInOwl:hasOBONamespace>GAZ</oboInOwl:hasOBONamespace>
        <oboInOwl:id>GAZ:00252284</oboInOwl:id>
        <rdfs:label>Hushirt Nuur</rdfs:label>
    </owl:NamedIndividual>
    


    <!-- http://purl.obolibrary.org/obo/GAZ_00252288 -->

    <owl:NamedIndividual rdf:about="http://purl.obolibrary.org/obo/GAZ_00252288">
        <obo:RO_0001025 rdf:resource="http://purl.obolibrary.org/obo/GAZ_00014875"/>
        <obo:IAO_0000115>A freshwater lake. Located on the Chinese border, 50 km NNE of Tamsagbulag,in extreme eastern Mongolia.</obo:IAO_0000115>
        <oboInOwl:hasOBONamespace>GAZ</oboInOwl:hasOBONamespace>
        <oboInOwl:id>GAZ:00252288</oboInOwl:id>
        <rdfs:label>Buyr Nuur</rdfs:label>
    </owl:NamedIndividual>
    


    <!-- http://purl.obolibrary.org/obo/GAZ_00252296 -->

    <owl:NamedIndividual rdf:about="http://purl.obolibrary.org/obo/GAZ_00252296">
        <obo:RO_0001025 rdf:resource="http://purl.obolibrary.org/obo/GAZ_00014868"/>
        <obo:RO_0001025 rdf:resource="http://purl.obolibrary.org/obo/GAZ_00252305"/>
        <obo:IAO_0000115>A seasonal lake. Located in the Gobi Valley of Lakes, about 60 km east of Boon Tsagaan Nuur and 125 km south of Bayankhongor, Bayankhongor Province.</obo:IAO_0000115>
        <oboInOwl:hasOBONamespace>GAZ</oboInOwl:hasOBONamespace>
        <oboInOwl:id>GAZ:00252296</oboInOwl:id>
        <rdfs:label>Adgiyn Tsagaan Nuur</rdfs:label>
    </owl:NamedIndividual>
    


    <!-- http://purl.obolibrary.org/obo/GAZ_00252299 -->

    <owl:NamedIndividual rdf:about="http://purl.obolibrary.org/obo/GAZ_00252299">
        <obo:RO_0001025 rdf:resource="http://purl.obolibrary.org/obo/GAZ_00014886"/>
        <obo:RO_0001025 rdf:resource="http://purl.obolibrary.org/obo/GAZ_00252305"/>
        <obo:IAO_0000115>A shallow, slightly saline lake with shores of mud, fine shingle and sand, in the same sandy depression as Orog Nuur, about 60 km to the east. Located in the Gobi Valley of Lakes at the foot of the Baga Bogd Masif of the Gobi-Altai, 160 km southwest of Arvayheer, Oeverkhangai Province.</obo:IAO_0000115>
        <oboInOwl:hasOBONamespace>GAZ</oboInOwl:hasOBONamespace>
        <oboInOwl:id>GAZ:00252299</oboInOwl:id>
        <rdfs:label>Tatsain Tsagaan Nuur</rdfs:label>
    </owl:NamedIndividual>
    


    <!-- http://purl.obolibrary.org/obo/GAZ_00252301 -->

    <owl:NamedIndividual rdf:about="http://purl.obolibrary.org/obo/GAZ_00252301">
        <obo:RO_0001025 rdf:resource="http://purl.obolibrary.org/obo/GAZ_00014882"/>
        <obo:RO_0001025 rdf:resource="http://purl.obolibrary.org/obo/GAZ_00252305"/>
        <obo:IAO_0000115>A shallow, slightly saline lake. It is the easternmost of the lakes in the Gobi Valley, about 120 km northwest of Dalandzadagad, Omnogovi Province.</obo:IAO_0000115>
        <oboInOwl:hasOBONamespace>GAZ</oboInOwl:hasOBONamespace>
        <oboInOwl:id>GAZ:00252301</oboInOwl:id>
        <rdfs:label>Ulaan Nuur</rdfs:label>
    </owl:NamedIndividual>
    


    <!-- http://purl.obolibrary.org/obo/GAZ_00252303 -->

    <owl:NamedIndividual rdf:about="http://purl.obolibrary.org/obo/GAZ_00252303">
        <obo:RO_0001025 rdf:resource="http://purl.obolibrary.org/obo/GAZ_00014878"/>
        <obo:IAO_0000115>A freshwater lake.</obo:IAO_0000115>
        <oboInOwl:hasOBONamespace>GAZ</oboInOwl:hasOBONamespace>
        <oboInOwl:id>GAZ:00252303</oboInOwl:id>
        <rdfs:label>Tal Nuur</rdfs:label>
    </owl:NamedIndividual>
    


    <!-- http://purl.obolibrary.org/obo/GAZ_00252304 -->

    <owl:NamedIndividual rdf:about="http://purl.obolibrary.org/obo/GAZ_00252304">
        <obo:RO_0001025 rdf:resource="http://purl.obolibrary.org/obo/GAZ_00014878"/>
        <obo:IAO_0000115>A freshwater lake.</obo:IAO_0000115>
        <oboInOwl:hasOBONamespace>GAZ</oboInOwl:hasOBONamespace>
        <oboInOwl:id>GAZ:00252304</oboInOwl:id>
        <rdfs:label>Tsagaan Nuur</rdfs:label>
    </owl:NamedIndividual>
    


    <!-- http://purl.obolibrary.org/obo/GAZ_00252305 -->

    <owl:NamedIndividual rdf:about="http://purl.obolibrary.org/obo/GAZ_00252305">
        <obo:RO_0001025 rdf:resource="http://purl.obolibrary.org/obo/GAZ_00057467"/>
        <obo:IAO_0000115>A region of the Gobi Desert that lies north of Alashan Plateau semi-desert, between the Gobi Altai range to the south and the Khangai Mountains to the north.</obo:IAO_0000115>
        <oboInOwl:hasOBONamespace>GAZ</oboInOwl:hasOBONamespace>
        <oboInOwl:id>GAZ:00252305</oboInOwl:id>
        <rdfs:label>Gobi Lakes Valley</rdfs:label>
    </owl:NamedIndividual>
    


    <!-- http://purl.obolibrary.org/obo/GAZ_00252306 -->

    <owl:NamedIndividual rdf:about="http://purl.obolibrary.org/obo/GAZ_00252306">
        <obo:RO_0001025 rdf:resource="http://purl.obolibrary.org/obo/GAZ_00014868"/>
        <obo:RO_0001025 rdf:resource="http://purl.obolibrary.org/obo/GAZ_00252305"/>
        <obo:IAO_0000115>A saline lake.</obo:IAO_0000115>
        <oboInOwl:hasOBONamespace>GAZ</oboInOwl:hasOBONamespace>
        <oboInOwl:id>GAZ:00252306</oboInOwl:id>
        <rdfs:label>Holboljin Nuur</rdfs:label>
    </owl:NamedIndividual>
    


    <!-- http://purl.obolibrary.org/obo/GAZ_00252307 -->

    <owl:NamedIndividual rdf:about="http://purl.obolibrary.org/obo/GAZ_00252307">
        <obo:RO_0001025 rdf:resource="http://purl.obolibrary.org/obo/GAZ_00014882"/>
        <obo:RO_0001025 rdf:resource="http://purl.obolibrary.org/obo/GAZ_00252305"/>
        <obo:IAO_0000115>A large inter-montane depression with salt pans and marshes.</obo:IAO_0000115>
        <oboInOwl:hasOBONamespace>GAZ</oboInOwl:hasOBONamespace>
        <oboInOwl:id>GAZ:00252307</oboInOwl:id>
        <rdfs:label>Hooloyn Nuur</rdfs:label>
    </owl:NamedIndividual>
    


    <!-- http://purl.obolibrary.org/obo/GAZ_00252308 -->

    <owl:NamedIndividual rdf:about="http://purl.obolibrary.org/obo/GAZ_00252308">
        <obo:RO_0001025 rdf:resource="http://purl.obolibrary.org/obo/GAZ_00014877"/>
        <obo:RO_0001025 rdf:resource="http://purl.obolibrary.org/obo/GAZ_00252276"/>
        <obo:IAO_0000115>A saline lake.</obo:IAO_0000115>
        <oboInOwl:hasOBONamespace>GAZ</oboInOwl:hasOBONamespace>
        <oboInOwl:id>GAZ:00252308</oboInOwl:id>
        <rdfs:label>Har Nuur</rdfs:label>
    </owl:NamedIndividual>
    


    <!-- http://purl.obolibrary.org/obo/GAZ_00252309 -->

    <owl:NamedIndividual rdf:about="http://purl.obolibrary.org/obo/GAZ_00252309">
        <obo:RO_0001025 rdf:resource="http://purl.obolibrary.org/obo/GAZ_00014877"/>
        <obo:RO_0001025 rdf:resource="http://purl.obolibrary.org/obo/GAZ_00252276"/>
        <obo:IAO_0000115>A saline lake.</obo:IAO_0000115>
        <oboInOwl:hasOBONamespace>GAZ</oboInOwl:hasOBONamespace>
        <oboInOwl:id>GAZ:00252309</oboInOwl:id>
        <rdfs:label>Oigon Nuur</rdfs:label>
    </owl:NamedIndividual>
    


    <!-- http://purl.obolibrary.org/obo/GAZ_00252310 -->

    <owl:NamedIndividual rdf:about="http://purl.obolibrary.org/obo/GAZ_00252310">
        <obo:RO_0001025 rdf:resource="http://purl.obolibrary.org/obo/GAZ_00014877"/>
        <obo:RO_0001025 rdf:resource="http://purl.obolibrary.org/obo/GAZ_00252276"/>
        <obo:IAO_0000115>A saline lake.</obo:IAO_0000115>
        <oboInOwl:hasOBONamespace>GAZ</oboInOwl:hasOBONamespace>
        <oboInOwl:id>GAZ:00252310</oboInOwl:id>
        <rdfs:label>Holboo Nuur</rdfs:label>
    </owl:NamedIndividual>
    


    <!-- http://purl.obolibrary.org/obo/GAZ_00252311 -->

    <owl:NamedIndividual rdf:about="http://purl.obolibrary.org/obo/GAZ_00252311">
        <obo:RO_0001025 rdf:resource="http://purl.obolibrary.org/obo/GAZ_00014885"/>
        <obo:RO_0001025 rdf:resource="http://purl.obolibrary.org/obo/GAZ_00252276"/>
        <obo:IAO_0000115>A saline lake.</obo:IAO_0000115>
        <oboInOwl:hasOBONamespace>GAZ</oboInOwl:hasOBONamespace>
        <oboInOwl:id>GAZ:00252311</oboInOwl:id>
        <rdfs:label>Bust Nuur</rdfs:label>
    </owl:NamedIndividual>
    


    <!-- http://purl.obolibrary.org/obo/GAZ_00252312 -->

    <owl:NamedIndividual rdf:about="http://purl.obolibrary.org/obo/GAZ_00252312">
        <obo:RO_0001025 rdf:resource="http://purl.obolibrary.org/obo/GAZ_00014885"/>
        <obo:RO_0001025 rdf:resource="http://purl.obolibrary.org/obo/GAZ_00252276"/>
        <obo:IAO_0000115>A freshwater lake.</obo:IAO_0000115>
        <oboInOwl:hasOBONamespace>GAZ</oboInOwl:hasOBONamespace>
        <oboInOwl:id>GAZ:00252312</oboInOwl:id>
        <rdfs:label>Jugnayn Nuur</rdfs:label>
    </owl:NamedIndividual>
    


    <!-- http://purl.obolibrary.org/obo/GAZ_00252313 -->

    <owl:NamedIndividual rdf:about="http://purl.obolibrary.org/obo/GAZ_00252313">
        <obo:RO_0001025 rdf:resource="http://purl.obolibrary.org/obo/GAZ_00014885"/>
        <obo:IAO_0000115>A freshwater lake.</obo:IAO_0000115>
        <oboInOwl:hasOBONamespace>GAZ</oboInOwl:hasOBONamespace>
        <oboInOwl:id>GAZ:00252313</oboInOwl:id>
        <rdfs:label>Dzuun Nuur</rdfs:label>
    </owl:NamedIndividual>
    


    <!-- http://purl.obolibrary.org/obo/GAZ_00252314 -->

    <owl:NamedIndividual rdf:about="http://purl.obolibrary.org/obo/GAZ_00252314">
        <obo:RO_0001025 rdf:resource="http://purl.obolibrary.org/obo/GAZ_00014874"/>
        <obo:IAO_0000115>A freshwater lake.</obo:IAO_0000115>
        <oboInOwl:hasOBONamespace>GAZ</oboInOwl:hasOBONamespace>
        <oboInOwl:id>GAZ:00252314</oboInOwl:id>
        <rdfs:label>Sharga Nuur</rdfs:label>
    </owl:NamedIndividual>
    


    <!-- http://purl.obolibrary.org/obo/GAZ_00252315 -->

    <owl:NamedIndividual rdf:about="http://purl.obolibrary.org/obo/GAZ_00252315">
        <obo:RO_0001025 rdf:resource="http://purl.obolibrary.org/obo/GAZ_00014869"/>
        <obo:IAO_0000115>A freshwater lake.</obo:IAO_0000115>
        <oboInOwl:hasOBONamespace>GAZ</oboInOwl:hasOBONamespace>
        <oboInOwl:id>GAZ:00252315</oboInOwl:id>
        <rdfs:label>Ih Tohom Nuur</rdfs:label>
    </owl:NamedIndividual>
    


    <!-- http://purl.obolibrary.org/obo/GAZ_00252316 -->

    <owl:NamedIndividual rdf:about="http://purl.obolibrary.org/obo/GAZ_00252316">
        <obo:RO_0001025 rdf:resource="http://purl.obolibrary.org/obo/GAZ_00014875"/>
        <obo:IAO_0000115>A freshwater lake.</obo:IAO_0000115>
        <oboInOwl:hasOBONamespace>GAZ</oboInOwl:hasOBONamespace>
        <oboInOwl:id>GAZ:00252316</oboInOwl:id>
        <rdfs:label>Hoh Nuur</rdfs:label>
    </owl:NamedIndividual>
    


    <!-- http://purl.obolibrary.org/obo/GAZ_00252317 -->

    <owl:NamedIndividual rdf:about="http://purl.obolibrary.org/obo/GAZ_00252317">
        <obo:RO_0001025 rdf:resource="http://purl.obolibrary.org/obo/GAZ_00014875"/>
        <obo:IAO_0000115>Two freshwater lakes.</obo:IAO_0000115>
        <oboInOwl:hasOBONamespace>GAZ</oboInOwl:hasOBONamespace>
        <oboInOwl:id>GAZ:00252317</oboInOwl:id>
        <rdfs:label>Melehiiteyn Nuur</rdfs:label>
    </owl:NamedIndividual>
    


    <!-- http://purl.obolibrary.org/obo/GAZ_00252318 -->

    <owl:NamedIndividual rdf:about="http://purl.obolibrary.org/obo/GAZ_00252318">
        <obo:RO_0001025 rdf:resource="http://purl.obolibrary.org/obo/GAZ_00014875"/>
        <obo:IAO_0000115>A freshwater lake. Located 20 km northeast of Tamsagbulag.</obo:IAO_0000115>
        <oboInOwl:hasOBONamespace>GAZ</oboInOwl:hasOBONamespace>
        <oboInOwl:id>GAZ:00252318</oboInOwl:id>
        <rdfs:label>Bulangiyn Shavar Nuur</rdfs:label>
    </owl:NamedIndividual>
    


    <!-- http://purl.obolibrary.org/obo/GAZ_00252319 -->

    <owl:NamedIndividual rdf:about="http://purl.obolibrary.org/obo/GAZ_00252319">
        <obo:RO_0001025 rdf:resource="http://purl.obolibrary.org/obo/GAZ_00008744"/>
        <obo:IAO_0000115>A river.</obo:IAO_0000115>
        <oboInOwl:hasOBONamespace>GAZ</oboInOwl:hasOBONamespace>
        <oboInOwl:id>GAZ:00252319</oboInOwl:id>
        <rdfs:label>Kyzyl-Khem</rdfs:label>
    </owl:NamedIndividual>
    


    <!-- 
    ///////////////////////////////////////////////////////////////////////////////////////
    //
    // Annotations
    //
    ///////////////////////////////////////////////////////////////////////////////////////
     -->

    <rdf:Description rdf:about="http://purl.obolibrary.org/obo/GAZ_00009465">
        <oboInOwl:hasOBONamespace>GAZ</oboInOwl:hasOBONamespace>
        <oboInOwl:id>GAZ:00009465</oboInOwl:id>
        <rdfs:label>Province (Mongolia)</rdfs:label>
    </rdf:Description>
    <rdf:Description rdf:about="http://purl.obolibrary.org/obo/GAZ_00014867">
        <rdfs:label>Dundgovi Province</rdfs:label>
        <obo:IAO_0000115>One of the 21 aimags (provinces) of Mongolia. It is located in the south of the country, approximately 245 km south of Ulaanbaatar. Its capital is Mandalgovi.</obo:IAO_0000115>
        <oboInOwl:hasOBONamespace>GAZ</oboInOwl:hasOBONamespace>
        <oboInOwl:id>GAZ:00014867</oboInOwl:id>
    </rdf:Description>
    <rdf:Description rdf:about="http://purl.obolibrary.org/obo/GAZ_00014868">
        <oboInOwl:id>GAZ:00014868</oboInOwl:id>
        <oboInOwl:hasOBONamespace>GAZ</oboInOwl:hasOBONamespace>
        <rdfs:label>Bayankhongor Province</rdfs:label>
        <obo:IAO_0000115>One of the 21 aimags of Mongolia. It is located in the south of the country. Its capital is Bayankhongor.</obo:IAO_0000115>
    </rdf:Description>
    <rdf:Description rdf:about="http://purl.obolibrary.org/obo/GAZ_00014869">
        <oboInOwl:hasOBONamespace>GAZ</oboInOwl:hasOBONamespace>
        <oboInOwl:id>GAZ:00014869</oboInOwl:id>
        <rdfs:label>Tov Province</rdfs:label>
        <obo:IAO_0000115>One of the 21 aimags (provinces) of Mongolia. The national capital Ulan Bator is located roughly at its center, but the city itself is administrated as an independent municipality.</obo:IAO_0000115>
    </rdf:Description>
    <rdf:Description rdf:about="http://purl.obolibrary.org/obo/GAZ_00014870">
        <oboInOwl:hasOBONamespace>GAZ</oboInOwl:hasOBONamespace>
        <oboInOwl:id>GAZ:00014870</oboInOwl:id>
        <rdfs:label>Dornogovi Province</rdfs:label>
        <obo:IAO_0000115>One of the 21 Aimags (provinces) of Mongolia. It is located in the southeast of the country.</obo:IAO_0000115>
    </rdf:Description>
    <rdf:Description rdf:about="http://purl.obolibrary.org/obo/GAZ_00014871">
        <oboInOwl:hasOBONamespace>GAZ</oboInOwl:hasOBONamespace>
        <rdfs:label>Govisumber Province</rdfs:label>
        <obo:IAO_0000115>One of the 21 aimags (provinces) of Mongolia. It is located in the center of the country. Its capital is Choir.</obo:IAO_0000115>
        <oboInOwl:id>GAZ:00014871</oboInOwl:id>
    </rdf:Description>
    <rdf:Description rdf:about="http://purl.obolibrary.org/obo/GAZ_00014872">
        <oboInOwl:hasOBONamespace>GAZ</oboInOwl:hasOBONamespace>
        <obo:IAO_0000115>One of the 21 aimags (provinces) of Mongolia. It is located in the north of the country. The Darkhan-Uul aimag with its four sum was carved out of the Selenge aimag in 1994.</obo:IAO_0000115>
        <rdfs:label>Darkhan-Uul Province</rdfs:label>
        <oboInOwl:id>GAZ:00014872</oboInOwl:id>
    </rdf:Description>
    <rdf:Description rdf:about="http://purl.obolibrary.org/obo/GAZ_00014873">
        <rdfs:label>Khentii Province</rdfs:label>
        <obo:IAO_0000115>One of the 21 aimags (provinces) of Mongolia, located in the east of the country. Its capital is Ondorkhaan. The aimag borders with Russia in the north. The neighbouring aimags are Darkhan-Uul in the northwest, Tov in the west, Govisumber in the southwest, Dornogovi in the south, Sukhbaatar in the southeast, and Dornod in the east. The border to Tov is divided by the city of Baganuur, an administrative exclave of Ulan Bator.</obo:IAO_0000115>
        <oboInOwl:hasOBONamespace>GAZ</oboInOwl:hasOBONamespace>
        <oboInOwl:id>GAZ:00014873</oboInOwl:id>
    </rdf:Description>
    <rdf:Description rdf:about="http://purl.obolibrary.org/obo/GAZ_00014874">
        <rdfs:label>Bulgan Province</rdfs:label>
        <oboInOwl:hasOBONamespace>GAZ</oboInOwl:hasOBONamespace>
        <obo:IAO_0000115>One of the 21 aimags (provinces) of Mongolia, located in northern Mongolia. The aimag is surrounded by the aimags Khovsgol in the northwest, Arkhangai in the southwest, Ovorkhangai in the south, Tov in the southeast, and Selenge in the northeast. The small Orkhon Aimag forms an enclave at the border to Selenge.</obo:IAO_0000115>
        <oboInOwl:id>GAZ:00014874</oboInOwl:id>
    </rdf:Description>
    <rdf:Description rdf:about="http://purl.obolibrary.org/obo/GAZ_00014875">
        <oboInOwl:id>GAZ:00014875</oboInOwl:id>
        <obo:IAO_0000115>The easternmost of the 21 aimags (provinces) of Mongolia. Its capital is Choibalsan.</obo:IAO_0000115>
        <rdfs:label>Dornod Province</rdfs:label>
        <oboInOwl:hasOBONamespace>GAZ</oboInOwl:hasOBONamespace>
    </rdf:Description>
    <rdf:Description rdf:about="http://purl.obolibrary.org/obo/GAZ_00014876">
        <oboInOwl:id>GAZ:00014876</oboInOwl:id>
        <rdfs:label>Uvs Province</rdfs:label>
        <oboInOwl:hasOBONamespace>GAZ</oboInOwl:hasOBONamespace>
        <obo:IAO_0000115>One of the 21 aimags (provinces) of Mongolia. It is located in the west of the country, 1336 km away from the national capital Ulan Bator. Its capital is Ulaangom. In the north the province borders the Russian Federation for 640 km, in the east 340 km of border lies between Uvs and Zavkhan province. In the south and west it borders with Khovd and Bayan-Olgii provinces for 200 km each.</obo:IAO_0000115>
    </rdf:Description>
    <rdf:Description rdf:about="http://purl.obolibrary.org/obo/GAZ_00014877">
        <oboInOwl:id>GAZ:00014877</oboInOwl:id>
        <oboInOwl:hasOBONamespace>GAZ</oboInOwl:hasOBONamespace>
        <rdfs:label>Zavkhan Province</rdfs:label>
        <obo:IAO_0000115>One of the 21 aimags (provinces) of Mongolia, located in the west of the country. Its capital is Uliastai.</obo:IAO_0000115>
    </rdf:Description>
    <rdf:Description rdf:about="http://purl.obolibrary.org/obo/GAZ_00014878">
        <rdfs:label>Bayan-Olgii Province</rdfs:label>
        <oboInOwl:hasOBONamespace>GAZ</oboInOwl:hasOBONamespace>
        <obo:IAO_0000115>The westernmost of the 21 aimags (provinces) of Mongolia. The aimag was established in 1940. The aimag is located in the extreme west of the country, and shares borders with both Russia and China. The border between the two neighbouring countries is very short here, though, and ends after about 40 km at the eastern end of Kazakhstan. Within Mongolia, the neighbouring aimags are Uvs in the north east and Khovd in the south east.</obo:IAO_0000115>
        <oboInOwl:id>GAZ:00014878</oboInOwl:id>
    </rdf:Description>
    <rdf:Description rdf:about="http://purl.obolibrary.org/obo/GAZ_00014879">
        <oboInOwl:hasOBONamespace>GAZ</oboInOwl:hasOBONamespace>
        <rdfs:label>Govi-Altai Province</rdfs:label>
        <oboInOwl:id>GAZ:00014879</oboInOwl:id>
        <obo:IAO_0000115>One of the 21 aimags (provinces) of Mongolia. It is located in the west of the country.</obo:IAO_0000115>
    </rdf:Description>
    <rdf:Description rdf:about="http://purl.obolibrary.org/obo/GAZ_00014880">
        <oboInOwl:hasOBONamespace>GAZ</oboInOwl:hasOBONamespace>
        <rdfs:label>Arkhangai Province</rdfs:label>
        <obo:IAO_0000115>One of the 21 Aimags (provinces) of Mongolia. It is located slightly west to the country&apos;s center, on the northern slopes of the Khangai Mountains. The Arkhangai aimag is located in the interior of the country and borders to the following other aimags: Bulgan (north east), Ovorkhangai (south east), Bayankhongor (south), Zavkhan (west), and Khovsgol (north west).</obo:IAO_0000115>
        <oboInOwl:id>GAZ:00014880</oboInOwl:id>
    </rdf:Description>
    <rdf:Description rdf:about="http://purl.obolibrary.org/obo/GAZ_00014881">
        <rdfs:label>Selenge Province</rdfs:label>
        <oboInOwl:hasOBONamespace>GAZ</oboInOwl:hasOBONamespace>
        <oboInOwl:id>GAZ:00014881</oboInOwl:id>
        <obo:IAO_0000115>One of the 21 aimags (provinces) of Mongolia, located in the north of the country. The capital is Sukhbaatar.</obo:IAO_0000115>
    </rdf:Description>
    <rdf:Description rdf:about="http://purl.obolibrary.org/obo/GAZ_00014882">
        <oboInOwl:hasOBONamespace>GAZ</oboInOwl:hasOBONamespace>
        <oboInOwl:id>GAZ:00014882</oboInOwl:id>
        <obo:IAO_0000115>An aimag (province) of Mongolia, located in the south of the country, in the Gobi Desert. The capital is Dalanzadgad.</obo:IAO_0000115>
        <rdfs:label>Omnogovi Province</rdfs:label>
    </rdf:Description>
    <rdf:Description rdf:about="http://purl.obolibrary.org/obo/GAZ_00014883">
        <obo:IAO_0000115>One of the 21 aimags (provinces) of Mongolia, located in the west of the country. Its capital is also named Khovd.</obo:IAO_0000115>
        <oboInOwl:hasOBONamespace>GAZ</oboInOwl:hasOBONamespace>
        <rdfs:label>Khovd Province</rdfs:label>
        <oboInOwl:id>GAZ:00014883</oboInOwl:id>
    </rdf:Description>
    <rdf:Description rdf:about="http://purl.obolibrary.org/obo/GAZ_00014884">
        <rdfs:label>Orkhon Province</rdfs:label>
        <obo:IAO_0000115>One of the 21 Aimags (provinces) of Mongolia, located in the north of the country. Its capital is Erdenet. Parts of the Orkhon Valley Cultural Landscape are situated in this province. This Aimag was cut out of Bulgan Aimag in 1994, to form a new entity together with its capital Erdenet, which had previously been administrated as a federal municipality.</obo:IAO_0000115>
        <oboInOwl:id>GAZ:00014884</oboInOwl:id>
        <oboInOwl:hasOBONamespace>GAZ</oboInOwl:hasOBONamespace>
    </rdf:Description>
    <rdf:Description rdf:about="http://purl.obolibrary.org/obo/GAZ_00014885">
        <obo:IAO_0000115>The northernmost of the 21 aimags (provinces) of Mongolia.</obo:IAO_0000115>
        <oboInOwl:id>GAZ:00014885</oboInOwl:id>
        <rdfs:label>Khovsgol Province</rdfs:label>
        <oboInOwl:hasOBONamespace>GAZ</oboInOwl:hasOBONamespace>
    </rdf:Description>
    <rdf:Description rdf:about="http://purl.obolibrary.org/obo/GAZ_00014886">
        <obo:IAO_0000115>One of the 21 aimags (provinces) of Mongolia, located in the south of the country. Its capital is Arvaikheer.</obo:IAO_0000115>
        <oboInOwl:id>GAZ:00014886</oboInOwl:id>
        <oboInOwl:hasOBONamespace>GAZ</oboInOwl:hasOBONamespace>
        <rdfs:label>Ovorkhangai Province</rdfs:label>
    </rdf:Description>
    <rdf:Description rdf:about="http://purl.obolibrary.org/obo/GAZ_00014887">
        <obo:IAO_0000115>One of the 21 aimags of Mongolia, located in the east of the country. Its capital is Baruun-Urt.</obo:IAO_0000115>
        <rdfs:label>Sukhbaatar Province</rdfs:label>
        <oboInOwl:id>GAZ:00014887</oboInOwl:id>
        <oboInOwl:hasOBONamespace>GAZ</oboInOwl:hasOBONamespace>
    </rdf:Description>
    <rdf:Description rdf:about="http://purl.obolibrary.org/obo/GAZ_00252209">
        <oboInOwl:id>GAZ:00252209</oboInOwl:id>
        <rdfs:label>Selenge River</rdfs:label>
        <oboInOwl:hasOBONamespace>GAZ</oboInOwl:hasOBONamespace>
        <obo:IAO_0000115>A river in Mongolia and Buryatia (Russia). Its source rivers are the Ideriin River and the Delgermoron. It flows into Lake Baikal and has a length of 992 km. The Selenga is the headwater of the Yenisei-Angara River.</obo:IAO_0000115>
    </rdf:Description>
</rdf:RDF>



<!-- Generated by the OWL API (version 4.5.6) https://github.com/owlcs/owlapi -->

