<?xml version="1.0"?>
<rdf:RDF xmlns="http://purl.obolibrary.org/obo/gaz/subsets/countries/Myanmar.owl#"
     xml:base="http://purl.obolibrary.org/obo/gaz/subsets/countries/Myanmar.owl"
     xmlns:obo="http://purl.obolibrary.org/obo/"
     xmlns:owl="http://www.w3.org/2002/07/owl#"
     xmlns:rdf="http://www.w3.org/1999/02/22-rdf-syntax-ns#"
     xmlns:xml="http://www.w3.org/XML/1998/namespace"
     xmlns:xsd="http://www.w3.org/2001/XMLSchema#"
     xmlns:rdfs="http://www.w3.org/2000/01/rdf-schema#"
     xmlns:oboInOwl="http://www.geneontology.org/formats/oboInOwl#">
    <owl:Ontology rdf:about="http://purl.obolibrary.org/obo/gaz/subsets/countries/Myanmar.owl">
        <owl:imports rdf:resource="http://purl.obolibrary.org/obo/gaz/imports/envo_import.owl"/>
        <owl:imports rdf:resource="http://purl.obolibrary.org/obo/gaz/imports/ro_import.owl"/>
    </owl:Ontology>
    


    <!-- 
    ///////////////////////////////////////////////////////////////////////////////////////
    //
    // Annotation properties
    //
    ///////////////////////////////////////////////////////////////////////////////////////
     -->

    


    <!-- http://purl.obolibrary.org/obo/IAO_0000115 -->

    <owl:AnnotationProperty rdf:about="http://purl.obolibrary.org/obo/IAO_0000115"/>
    


    <!-- http://www.geneontology.org/formats/oboInOwl#hasOBONamespace -->

    <owl:AnnotationProperty rdf:about="http://www.geneontology.org/formats/oboInOwl#hasOBONamespace"/>
    


    <!-- http://www.geneontology.org/formats/oboInOwl#id -->

    <owl:AnnotationProperty rdf:about="http://www.geneontology.org/formats/oboInOwl#id"/>
    


    <!-- 
    ///////////////////////////////////////////////////////////////////////////////////////
    //
    // Object Properties
    //
    ///////////////////////////////////////////////////////////////////////////////////////
     -->

    


    <!-- http://purl.obolibrary.org/obo/RO_0001025 -->

    <owl:ObjectProperty rdf:about="http://purl.obolibrary.org/obo/RO_0001025"/>
    


    <!-- 
    ///////////////////////////////////////////////////////////////////////////////////////
    //
    // Classes
    //
    ///////////////////////////////////////////////////////////////////////////////////////
     -->

    


    <!-- http://purl.obolibrary.org/obo/ENVO_00000004 -->

    <owl:Class rdf:about="http://purl.obolibrary.org/obo/ENVO_00000004"/>
    


    <!-- http://purl.obolibrary.org/obo/ENVO_00000009 -->

    <owl:Class rdf:about="http://purl.obolibrary.org/obo/ENVO_00000009"/>
    


    <!-- http://purl.obolibrary.org/obo/ENVO_00000106 -->

    <owl:Class rdf:about="http://purl.obolibrary.org/obo/ENVO_00000106"/>
    


    <!-- http://purl.obolibrary.org/obo/ENVO_00000220 -->

    <owl:Class rdf:about="http://purl.obolibrary.org/obo/ENVO_00000220"/>
    


    <!-- http://purl.obolibrary.org/obo/ENVO_00000305 -->

    <owl:Class rdf:about="http://purl.obolibrary.org/obo/ENVO_00000305"/>
    


    <!-- http://purl.obolibrary.org/obo/ENVO_00000475 -->

    <owl:Class rdf:about="http://purl.obolibrary.org/obo/ENVO_00000475"/>
    


    <!-- http://purl.obolibrary.org/obo/ENVO_00000856 -->

    <owl:Class rdf:about="http://purl.obolibrary.org/obo/ENVO_00000856"/>
    


    <!-- http://purl.obolibrary.org/obo/GAZ_00002782 -->

    <owl:Class rdf:about="http://purl.obolibrary.org/obo/GAZ_00002782"/>
    


    <!-- http://purl.obolibrary.org/obo/GAZ_02000000 -->

    <owl:Class rdf:about="http://purl.obolibrary.org/obo/GAZ_02000000">
        <rdfs:subClassOf rdf:resource="http://purl.obolibrary.org/obo/GAZ_00002782"/>
    </owl:Class>
    


    <!-- http://purl.obolibrary.org/obo/GAZ_02000001 -->

    <owl:Class rdf:about="http://purl.obolibrary.org/obo/GAZ_02000001">
        <rdfs:subClassOf rdf:resource="http://purl.obolibrary.org/obo/GAZ_00002782"/>
    </owl:Class>
    


    <!-- http://purl.obolibrary.org/obo/GAZ_02000002 -->

    <owl:Class rdf:about="http://purl.obolibrary.org/obo/GAZ_02000002">
        <rdfs:subClassOf rdf:resource="http://purl.obolibrary.org/obo/GAZ_00002782"/>
    </owl:Class>
    


    <!-- http://purl.obolibrary.org/obo/GAZ_02000003 -->

    <owl:Class rdf:about="http://purl.obolibrary.org/obo/GAZ_02000003">
        <rdfs:subClassOf rdf:resource="http://purl.obolibrary.org/obo/GAZ_00002782"/>
    </owl:Class>
    


    <!-- http://purl.obolibrary.org/obo/GAZ_02000004 -->

    <owl:Class rdf:about="http://purl.obolibrary.org/obo/GAZ_02000004">
        <rdfs:subClassOf rdf:resource="http://purl.obolibrary.org/obo/GAZ_00002782"/>
    </owl:Class>
    


    <!-- http://purl.obolibrary.org/obo/GAZ_02000005 -->

    <owl:Class rdf:about="http://purl.obolibrary.org/obo/GAZ_02000005">
        <rdfs:subClassOf rdf:resource="http://purl.obolibrary.org/obo/GAZ_00002782"/>
    </owl:Class>
    


    <!-- http://purl.obolibrary.org/obo/GAZ_02000006 -->

    <owl:Class rdf:about="http://purl.obolibrary.org/obo/GAZ_02000006">
        <rdfs:subClassOf rdf:resource="http://purl.obolibrary.org/obo/GAZ_00002782"/>
    </owl:Class>
    


    <!-- http://purl.obolibrary.org/obo/GAZ_02000007 -->

    <owl:Class rdf:about="http://purl.obolibrary.org/obo/GAZ_02000007">
        <rdfs:subClassOf rdf:resource="http://purl.obolibrary.org/obo/GAZ_02000896"/>
    </owl:Class>
    


    <!-- http://purl.obolibrary.org/obo/GAZ_02000008 -->

    <owl:Class rdf:about="http://purl.obolibrary.org/obo/GAZ_02000008">
        <rdfs:subClassOf rdf:resource="http://purl.obolibrary.org/obo/GAZ_02000896"/>
    </owl:Class>
    


    <!-- http://purl.obolibrary.org/obo/GAZ_02000009 -->

    <owl:Class rdf:about="http://purl.obolibrary.org/obo/GAZ_02000009">
        <rdfs:subClassOf rdf:resource="http://purl.obolibrary.org/obo/GAZ_02000896"/>
    </owl:Class>
    


    <!-- http://purl.obolibrary.org/obo/GAZ_02000010 -->

    <owl:Class rdf:about="http://purl.obolibrary.org/obo/GAZ_02000010">
        <rdfs:subClassOf rdf:resource="http://purl.obolibrary.org/obo/GAZ_02000896"/>
    </owl:Class>
    


    <!-- http://purl.obolibrary.org/obo/GAZ_02000011 -->

    <owl:Class rdf:about="http://purl.obolibrary.org/obo/GAZ_02000011">
        <rdfs:subClassOf rdf:resource="http://purl.obolibrary.org/obo/GAZ_02000896"/>
    </owl:Class>
    


    <!-- http://purl.obolibrary.org/obo/GAZ_02000012 -->

    <owl:Class rdf:about="http://purl.obolibrary.org/obo/GAZ_02000012">
        <rdfs:subClassOf rdf:resource="http://purl.obolibrary.org/obo/GAZ_02000896"/>
    </owl:Class>
    


    <!-- http://purl.obolibrary.org/obo/GAZ_02000013 -->

    <owl:Class rdf:about="http://purl.obolibrary.org/obo/GAZ_02000013">
        <rdfs:subClassOf rdf:resource="http://purl.obolibrary.org/obo/GAZ_02000896"/>
    </owl:Class>
    


    <!-- http://purl.obolibrary.org/obo/GAZ_02000896 -->

    <owl:Class rdf:about="http://purl.obolibrary.org/obo/GAZ_02000896"/>
    


    <!-- 
    ///////////////////////////////////////////////////////////////////////////////////////
    //
    // Individuals
    //
    ///////////////////////////////////////////////////////////////////////////////////////
     -->

    


    <!-- http://purl.obolibrary.org/obo/GAZ_00002782 -->

    <owl:NamedIndividual rdf:about="http://purl.obolibrary.org/obo/GAZ_00002782">
        <obo:RO_0001025 rdf:resource="http://purl.obolibrary.org/obo/GAZ_00006899"/>
    </owl:NamedIndividual>
    


    <!-- http://purl.obolibrary.org/obo/GAZ_00006899 -->

    <owl:NamedIndividual rdf:about="http://purl.obolibrary.org/obo/GAZ_00006899">
        <rdf:type rdf:resource="http://purl.obolibrary.org/obo/ENVO_00000009"/>
        <obo:IAO_0000115>A country in SE Asia that is bordered by China on the north, Laos on the east, Thailand on the southeast, Bangladesh on the west, and India on the northwest, with the Bay of Bengal to the southwest. Myanmar is divided into seven states and seven divisions. The administrative divisions are further subdivided into districts, which are further subdivided into townships, wards, and villages.</obo:IAO_0000115>
        <oboInOwl:hasOBONamespace>GAZ</oboInOwl:hasOBONamespace>
        <oboInOwl:id>GAZ:00006899</oboInOwl:id>
        <rdfs:label>Myanmar</rdfs:label>
    </owl:NamedIndividual>
    


    <!-- http://purl.obolibrary.org/obo/GAZ_00017493 -->

    <owl:NamedIndividual rdf:about="http://purl.obolibrary.org/obo/GAZ_00017493">
        <obo:RO_0001025 rdf:resource="http://purl.obolibrary.org/obo/GAZ_02000000"/>
        <obo:IAO_0000115>An archipelago in far southern Myanmar (Burma). It consists of more than 800 islands, varying in size from very small to hundreds of km2, all lying in the Andaman Sea off the western shore of the Malay Peninsula near its landward (northern) end where it joins the rest of Indochina.</obo:IAO_0000115>
        <oboInOwl:hasOBONamespace>GAZ</oboInOwl:hasOBONamespace>
        <oboInOwl:id>GAZ:00017493</oboInOwl:id>
        <rdfs:label>Mergui Archipelago</rdfs:label>
    </owl:NamedIndividual>
    


    <!-- http://purl.obolibrary.org/obo/GAZ_00025499 -->

    <owl:NamedIndividual rdf:about="http://purl.obolibrary.org/obo/GAZ_00025499">
        <rdf:type rdf:resource="http://purl.obolibrary.org/obo/ENVO_00000004"/>
        <obo:RO_0001025 rdf:resource="http://purl.obolibrary.org/obo/GAZ_02000002"/>
        <obo:IAO_0000115>A district of the Ayeyarwady Division in south western Myanmar.</obo:IAO_0000115>
        <oboInOwl:hasOBONamespace>GAZ</oboInOwl:hasOBONamespace>
        <oboInOwl:id>GAZ:00025499</oboInOwl:id>
        <rdfs:label>Myaungmya District</rdfs:label>
    </owl:NamedIndividual>
    


    <!-- http://purl.obolibrary.org/obo/GAZ_00025500 -->

    <owl:NamedIndividual rdf:about="http://purl.obolibrary.org/obo/GAZ_00025500">
        <rdf:type rdf:resource="http://purl.obolibrary.org/obo/ENVO_00000004"/>
        <obo:RO_0001025 rdf:resource="http://purl.obolibrary.org/obo/GAZ_02000002"/>
        <obo:IAO_0000115>A district of the Ayeyawady Division in south western Myanmar. It is located around the city of Pathein and includes the urban area of it.</obo:IAO_0000115>
        <oboInOwl:hasOBONamespace>GAZ</oboInOwl:hasOBONamespace>
        <oboInOwl:id>GAZ:00025500</oboInOwl:id>
        <rdfs:label>Pathein District</rdfs:label>
    </owl:NamedIndividual>
    


    <!-- http://purl.obolibrary.org/obo/GAZ_00025501 -->

    <owl:NamedIndividual rdf:about="http://purl.obolibrary.org/obo/GAZ_00025501">
        <rdf:type rdf:resource="http://purl.obolibrary.org/obo/ENVO_00000004"/>
        <obo:RO_0001025 rdf:resource="http://purl.obolibrary.org/obo/GAZ_02000002"/>
        <obo:IAO_0000115>A district of the Ayeyarwady Division in south western Myanmar.</obo:IAO_0000115>
        <oboInOwl:hasOBONamespace>GAZ</oboInOwl:hasOBONamespace>
        <oboInOwl:id>GAZ:00025501</oboInOwl:id>
        <rdfs:label>Pyapon District</rdfs:label>
    </owl:NamedIndividual>
    


    <!-- http://purl.obolibrary.org/obo/GAZ_00025502 -->

    <owl:NamedIndividual rdf:about="http://purl.obolibrary.org/obo/GAZ_00025502">
        <rdf:type rdf:resource="http://purl.obolibrary.org/obo/ENVO_00000004"/>
        <obo:RO_0001025 rdf:resource="http://purl.obolibrary.org/obo/GAZ_02000002"/>
        <obo:IAO_0000115>A district of the Ayeyarwady Division in south western Myanmar.</obo:IAO_0000115>
        <oboInOwl:hasOBONamespace>GAZ</oboInOwl:hasOBONamespace>
        <oboInOwl:id>GAZ:00025502</oboInOwl:id>
        <rdfs:label>Ma-Ubin District</rdfs:label>
    </owl:NamedIndividual>
    


    <!-- http://purl.obolibrary.org/obo/GAZ_00025503 -->

    <owl:NamedIndividual rdf:about="http://purl.obolibrary.org/obo/GAZ_00025503">
        <rdf:type rdf:resource="http://purl.obolibrary.org/obo/ENVO_00000004"/>
        <obo:RO_0001025 rdf:resource="http://purl.obolibrary.org/obo/GAZ_02000002"/>
        <obo:IAO_0000115>A district of the Ayeyarwady Division in south western Myanmar.</obo:IAO_0000115>
        <oboInOwl:hasOBONamespace>GAZ</oboInOwl:hasOBONamespace>
        <oboInOwl:id>GAZ:00025503</oboInOwl:id>
        <rdfs:label>Hinthada District</rdfs:label>
    </owl:NamedIndividual>
    


    <!-- http://purl.obolibrary.org/obo/GAZ_00025504 -->

    <owl:NamedIndividual rdf:about="http://purl.obolibrary.org/obo/GAZ_00025504">
        <rdf:type rdf:resource="http://purl.obolibrary.org/obo/ENVO_00000004"/>
        <obo:RO_0001025 rdf:resource="http://purl.obolibrary.org/obo/GAZ_02000004"/>
        <obo:IAO_0000115>A district of the Bago Division, Myanmar.</obo:IAO_0000115>
        <oboInOwl:hasOBONamespace>GAZ</oboInOwl:hasOBONamespace>
        <oboInOwl:id>GAZ:00025504</oboInOwl:id>
        <rdfs:label>Pyay District</rdfs:label>
    </owl:NamedIndividual>
    


    <!-- http://purl.obolibrary.org/obo/GAZ_00025505 -->

    <owl:NamedIndividual rdf:about="http://purl.obolibrary.org/obo/GAZ_00025505">
        <rdf:type rdf:resource="http://purl.obolibrary.org/obo/ENVO_00000004"/>
        <obo:RO_0001025 rdf:resource="http://purl.obolibrary.org/obo/GAZ_02000004"/>
        <obo:IAO_0000115>A district of the Bago Division, Myanmar.</obo:IAO_0000115>
        <oboInOwl:hasOBONamespace>GAZ</oboInOwl:hasOBONamespace>
        <oboInOwl:id>GAZ:00025505</oboInOwl:id>
        <rdfs:label>Bago District</rdfs:label>
    </owl:NamedIndividual>
    


    <!-- http://purl.obolibrary.org/obo/GAZ_00025506 -->

    <owl:NamedIndividual rdf:about="http://purl.obolibrary.org/obo/GAZ_00025506">
        <rdf:type rdf:resource="http://purl.obolibrary.org/obo/ENVO_00000004"/>
        <obo:RO_0001025 rdf:resource="http://purl.obolibrary.org/obo/GAZ_02000004"/>
        <obo:IAO_0000115>A district of the Bago Division, Myanmar.</obo:IAO_0000115>
        <oboInOwl:hasOBONamespace>GAZ</oboInOwl:hasOBONamespace>
        <oboInOwl:id>GAZ:00025506</oboInOwl:id>
        <rdfs:label>Taungoo District</rdfs:label>
    </owl:NamedIndividual>
    


    <!-- http://purl.obolibrary.org/obo/GAZ_00025507 -->

    <owl:NamedIndividual rdf:about="http://purl.obolibrary.org/obo/GAZ_00025507">
        <rdf:type rdf:resource="http://purl.obolibrary.org/obo/ENVO_00000004"/>
        <obo:RO_0001025 rdf:resource="http://purl.obolibrary.org/obo/GAZ_02000004"/>
        <obo:IAO_0000115>A district of the Bago Division, Myanmar.</obo:IAO_0000115>
        <oboInOwl:hasOBONamespace>GAZ</oboInOwl:hasOBONamespace>
        <oboInOwl:id>GAZ:00025507</oboInOwl:id>
        <rdfs:label>Thayawady District</rdfs:label>
    </owl:NamedIndividual>
    


    <!-- http://purl.obolibrary.org/obo/GAZ_00025508 -->

    <owl:NamedIndividual rdf:about="http://purl.obolibrary.org/obo/GAZ_00025508">
        <rdf:type rdf:resource="http://purl.obolibrary.org/obo/ENVO_00000004"/>
        <obo:RO_0001025 rdf:resource="http://purl.obolibrary.org/obo/GAZ_02000005"/>
        <obo:IAO_0000115>A district of the Magway Division in central Myanmar.</obo:IAO_0000115>
        <oboInOwl:hasOBONamespace>GAZ</oboInOwl:hasOBONamespace>
        <oboInOwl:id>GAZ:00025508</oboInOwl:id>
        <rdfs:label>Thayetmyo District</rdfs:label>
    </owl:NamedIndividual>
    


    <!-- http://purl.obolibrary.org/obo/GAZ_00025509 -->

    <owl:NamedIndividual rdf:about="http://purl.obolibrary.org/obo/GAZ_00025509">
        <rdf:type rdf:resource="http://purl.obolibrary.org/obo/ENVO_00000004"/>
        <obo:RO_0001025 rdf:resource="http://purl.obolibrary.org/obo/GAZ_02000005"/>
        <obo:IAO_0000115>A district of the Magway Division in central Myanmar.</obo:IAO_0000115>
        <oboInOwl:hasOBONamespace>GAZ</oboInOwl:hasOBONamespace>
        <oboInOwl:id>GAZ:00025509</oboInOwl:id>
        <rdfs:label>Gangaw District</rdfs:label>
    </owl:NamedIndividual>
    


    <!-- http://purl.obolibrary.org/obo/GAZ_00025510 -->

    <owl:NamedIndividual rdf:about="http://purl.obolibrary.org/obo/GAZ_00025510">
        <rdf:type rdf:resource="http://purl.obolibrary.org/obo/ENVO_00000004"/>
        <obo:RO_0001025 rdf:resource="http://purl.obolibrary.org/obo/GAZ_02000005"/>
        <obo:IAO_0000115>A district of the Magway Division in central Myanmar.</obo:IAO_0000115>
        <oboInOwl:hasOBONamespace>GAZ</oboInOwl:hasOBONamespace>
        <oboInOwl:id>GAZ:00025510</oboInOwl:id>
        <rdfs:label>Pakokku District</rdfs:label>
    </owl:NamedIndividual>
    


    <!-- http://purl.obolibrary.org/obo/GAZ_00025511 -->

    <owl:NamedIndividual rdf:about="http://purl.obolibrary.org/obo/GAZ_00025511">
        <rdf:type rdf:resource="http://purl.obolibrary.org/obo/ENVO_00000004"/>
        <obo:RO_0001025 rdf:resource="http://purl.obolibrary.org/obo/GAZ_02000005"/>
        <obo:IAO_0000115>A district of the Magway Division in central Myanmar.</obo:IAO_0000115>
        <oboInOwl:hasOBONamespace>GAZ</oboInOwl:hasOBONamespace>
        <oboInOwl:id>GAZ:00025511</oboInOwl:id>
        <rdfs:label>Magwe District</rdfs:label>
    </owl:NamedIndividual>
    


    <!-- http://purl.obolibrary.org/obo/GAZ_00025512 -->

    <owl:NamedIndividual rdf:about="http://purl.obolibrary.org/obo/GAZ_00025512">
        <rdf:type rdf:resource="http://purl.obolibrary.org/obo/ENVO_00000004"/>
        <obo:RO_0001025 rdf:resource="http://purl.obolibrary.org/obo/GAZ_02000005"/>
        <obo:IAO_0000115>A district of the Magway Division in central Myanmar.</obo:IAO_0000115>
        <oboInOwl:hasOBONamespace>GAZ</oboInOwl:hasOBONamespace>
        <oboInOwl:id>GAZ:00025512</oboInOwl:id>
        <rdfs:label>Minbu District</rdfs:label>
    </owl:NamedIndividual>
    


    <!-- http://purl.obolibrary.org/obo/GAZ_00025513 -->

    <owl:NamedIndividual rdf:about="http://purl.obolibrary.org/obo/GAZ_00025513">
        <rdf:type rdf:resource="http://purl.obolibrary.org/obo/ENVO_00000004"/>
        <obo:RO_0001025 rdf:resource="http://purl.obolibrary.org/obo/GAZ_02000003"/>
        <obo:IAO_0000115>A district of Sagaing Division, Myanmar.</obo:IAO_0000115>
        <oboInOwl:hasOBONamespace>GAZ</oboInOwl:hasOBONamespace>
        <oboInOwl:id>GAZ:00025513</oboInOwl:id>
        <rdfs:label>Shwebo District</rdfs:label>
    </owl:NamedIndividual>
    


    <!-- http://purl.obolibrary.org/obo/GAZ_00025514 -->

    <owl:NamedIndividual rdf:about="http://purl.obolibrary.org/obo/GAZ_00025514">
        <rdf:type rdf:resource="http://purl.obolibrary.org/obo/ENVO_00000004"/>
        <obo:RO_0001025 rdf:resource="http://purl.obolibrary.org/obo/GAZ_02000003"/>
        <obo:IAO_0000115>A district of Sagaing Division, Myanmar.</obo:IAO_0000115>
        <oboInOwl:hasOBONamespace>GAZ</oboInOwl:hasOBONamespace>
        <oboInOwl:id>GAZ:00025514</oboInOwl:id>
        <rdfs:label>Monywa District</rdfs:label>
    </owl:NamedIndividual>
    


    <!-- http://purl.obolibrary.org/obo/GAZ_00025515 -->

    <owl:NamedIndividual rdf:about="http://purl.obolibrary.org/obo/GAZ_00025515">
        <rdf:type rdf:resource="http://purl.obolibrary.org/obo/ENVO_00000004"/>
        <obo:RO_0001025 rdf:resource="http://purl.obolibrary.org/obo/GAZ_02000003"/>
        <obo:IAO_0000115>A district of Sagaing Division, Myanmar.</obo:IAO_0000115>
        <oboInOwl:hasOBONamespace>GAZ</oboInOwl:hasOBONamespace>
        <oboInOwl:id>GAZ:00025515</oboInOwl:id>
        <rdfs:label>Hkamti District</rdfs:label>
    </owl:NamedIndividual>
    


    <!-- http://purl.obolibrary.org/obo/GAZ_00025516 -->

    <owl:NamedIndividual rdf:about="http://purl.obolibrary.org/obo/GAZ_00025516">
        <rdf:type rdf:resource="http://purl.obolibrary.org/obo/ENVO_00000004"/>
        <obo:RO_0001025 rdf:resource="http://purl.obolibrary.org/obo/GAZ_02000003"/>
        <obo:IAO_0000115>A district of Sagaing Division, Myanmar.</obo:IAO_0000115>
        <oboInOwl:hasOBONamespace>GAZ</oboInOwl:hasOBONamespace>
        <oboInOwl:id>GAZ:00025516</oboInOwl:id>
        <rdfs:label>Kale District</rdfs:label>
    </owl:NamedIndividual>
    


    <!-- http://purl.obolibrary.org/obo/GAZ_00025517 -->

    <owl:NamedIndividual rdf:about="http://purl.obolibrary.org/obo/GAZ_00025517">
        <rdf:type rdf:resource="http://purl.obolibrary.org/obo/ENVO_00000004"/>
        <obo:RO_0001025 rdf:resource="http://purl.obolibrary.org/obo/GAZ_02000003"/>
        <obo:IAO_0000115>A district of Sagaing Division, Myanmar.</obo:IAO_0000115>
        <oboInOwl:hasOBONamespace>GAZ</oboInOwl:hasOBONamespace>
        <oboInOwl:id>GAZ:00025517</oboInOwl:id>
        <rdfs:label>Mawlaik District</rdfs:label>
    </owl:NamedIndividual>
    


    <!-- http://purl.obolibrary.org/obo/GAZ_00025518 -->

    <owl:NamedIndividual rdf:about="http://purl.obolibrary.org/obo/GAZ_00025518">
        <rdf:type rdf:resource="http://purl.obolibrary.org/obo/ENVO_00000004"/>
        <obo:RO_0001025 rdf:resource="http://purl.obolibrary.org/obo/GAZ_02000003"/>
        <obo:IAO_0000115>A district of Sagaing Division, Myanmar.</obo:IAO_0000115>
        <oboInOwl:hasOBONamespace>GAZ</oboInOwl:hasOBONamespace>
        <oboInOwl:id>GAZ:00025518</oboInOwl:id>
        <rdfs:label>Katha District</rdfs:label>
    </owl:NamedIndividual>
    


    <!-- http://purl.obolibrary.org/obo/GAZ_00025519 -->

    <owl:NamedIndividual rdf:about="http://purl.obolibrary.org/obo/GAZ_00025519">
        <rdf:type rdf:resource="http://purl.obolibrary.org/obo/ENVO_00000004"/>
        <obo:RO_0001025 rdf:resource="http://purl.obolibrary.org/obo/GAZ_02000003"/>
        <obo:IAO_0000115>A district of Sagaing Division, Myanmar.</obo:IAO_0000115>
        <oboInOwl:hasOBONamespace>GAZ</oboInOwl:hasOBONamespace>
        <oboInOwl:id>GAZ:00025519</oboInOwl:id>
        <rdfs:label>Sagaing District</rdfs:label>
    </owl:NamedIndividual>
    


    <!-- http://purl.obolibrary.org/obo/GAZ_00025520 -->

    <owl:NamedIndividual rdf:about="http://purl.obolibrary.org/obo/GAZ_00025520">
        <rdf:type rdf:resource="http://purl.obolibrary.org/obo/ENVO_00000004"/>
        <obo:RO_0001025 rdf:resource="http://purl.obolibrary.org/obo/GAZ_02000003"/>
        <obo:IAO_0000115>A district of Sagaing Division, Myanmar.</obo:IAO_0000115>
        <oboInOwl:hasOBONamespace>GAZ</oboInOwl:hasOBONamespace>
        <oboInOwl:id>GAZ:00025520</oboInOwl:id>
        <rdfs:label>Tamu District</rdfs:label>
    </owl:NamedIndividual>
    


    <!-- http://purl.obolibrary.org/obo/GAZ_00025526 -->

    <owl:NamedIndividual rdf:about="http://purl.obolibrary.org/obo/GAZ_00025526">
        <rdf:type rdf:resource="http://purl.obolibrary.org/obo/ENVO_00000004"/>
        <obo:RO_0001025 rdf:resource="http://purl.obolibrary.org/obo/GAZ_02000006"/>
        <obo:IAO_0000115>A district of Yangon Division.</obo:IAO_0000115>
        <oboInOwl:hasOBONamespace>GAZ</oboInOwl:hasOBONamespace>
        <oboInOwl:id>GAZ:00025526</oboInOwl:id>
        <rdfs:label>Yangon East District</rdfs:label>
    </owl:NamedIndividual>
    


    <!-- http://purl.obolibrary.org/obo/GAZ_00025527 -->

    <owl:NamedIndividual rdf:about="http://purl.obolibrary.org/obo/GAZ_00025527">
        <rdf:type rdf:resource="http://purl.obolibrary.org/obo/ENVO_00000004"/>
        <obo:RO_0001025 rdf:resource="http://purl.obolibrary.org/obo/GAZ_02000006"/>
        <obo:IAO_0000115>A district of Yangon Division.</obo:IAO_0000115>
        <oboInOwl:hasOBONamespace>GAZ</oboInOwl:hasOBONamespace>
        <oboInOwl:id>GAZ:00025527</oboInOwl:id>
        <rdfs:label>Yangon West District</rdfs:label>
    </owl:NamedIndividual>
    


    <!-- http://purl.obolibrary.org/obo/GAZ_00025528 -->

    <owl:NamedIndividual rdf:about="http://purl.obolibrary.org/obo/GAZ_00025528">
        <rdf:type rdf:resource="http://purl.obolibrary.org/obo/ENVO_00000004"/>
        <obo:RO_0001025 rdf:resource="http://purl.obolibrary.org/obo/GAZ_02000006"/>
        <obo:IAO_0000115>A district of Yangon Division.</obo:IAO_0000115>
        <oboInOwl:hasOBONamespace>GAZ</oboInOwl:hasOBONamespace>
        <oboInOwl:id>GAZ:00025528</oboInOwl:id>
        <rdfs:label>Yangon South District</rdfs:label>
    </owl:NamedIndividual>
    


    <!-- http://purl.obolibrary.org/obo/GAZ_00025529 -->

    <owl:NamedIndividual rdf:about="http://purl.obolibrary.org/obo/GAZ_00025529">
        <rdf:type rdf:resource="http://purl.obolibrary.org/obo/ENVO_00000004"/>
        <obo:RO_0001025 rdf:resource="http://purl.obolibrary.org/obo/GAZ_02000006"/>
        <obo:IAO_0000115>A district of Yangon Division.</obo:IAO_0000115>
        <oboInOwl:hasOBONamespace>GAZ</oboInOwl:hasOBONamespace>
        <oboInOwl:id>GAZ:00025529</oboInOwl:id>
        <rdfs:label>Yangon North District</rdfs:label>
    </owl:NamedIndividual>
    


    <!-- http://purl.obolibrary.org/obo/GAZ_00025530 -->

    <owl:NamedIndividual rdf:about="http://purl.obolibrary.org/obo/GAZ_00025530">
        <rdf:type rdf:resource="http://purl.obolibrary.org/obo/ENVO_00000004"/>
        <obo:RO_0001025 rdf:resource="http://purl.obolibrary.org/obo/GAZ_02000001"/>
        <obo:IAO_0000115>A district of the Mandalay Division in central Burma.</obo:IAO_0000115>
        <oboInOwl:hasOBONamespace>GAZ</oboInOwl:hasOBONamespace>
        <oboInOwl:id>GAZ:00025530</oboInOwl:id>
        <rdfs:label>Kyaukse District</rdfs:label>
    </owl:NamedIndividual>
    


    <!-- http://purl.obolibrary.org/obo/GAZ_00025531 -->

    <owl:NamedIndividual rdf:about="http://purl.obolibrary.org/obo/GAZ_00025531">
        <rdf:type rdf:resource="http://purl.obolibrary.org/obo/ENVO_00000004"/>
        <obo:RO_0001025 rdf:resource="http://purl.obolibrary.org/obo/GAZ_02000001"/>
        <obo:IAO_0000115>A district of the Mandalay Division in central Burma. It is located around the city of Mandalay and includes the urban area of it.</obo:IAO_0000115>
        <oboInOwl:hasOBONamespace>GAZ</oboInOwl:hasOBONamespace>
        <oboInOwl:id>GAZ:00025531</oboInOwl:id>
        <rdfs:label>Mandalay District</rdfs:label>
    </owl:NamedIndividual>
    


    <!-- http://purl.obolibrary.org/obo/GAZ_00025532 -->

    <owl:NamedIndividual rdf:about="http://purl.obolibrary.org/obo/GAZ_00025532">
        <rdf:type rdf:resource="http://purl.obolibrary.org/obo/ENVO_00000004"/>
        <obo:RO_0001025 rdf:resource="http://purl.obolibrary.org/obo/GAZ_02000001"/>
        <obo:IAO_0000115>A district of the Mandalay Division in central Burma.</obo:IAO_0000115>
        <oboInOwl:hasOBONamespace>GAZ</oboInOwl:hasOBONamespace>
        <oboInOwl:id>GAZ:00025532</oboInOwl:id>
        <rdfs:label>Meiktila District</rdfs:label>
    </owl:NamedIndividual>
    


    <!-- http://purl.obolibrary.org/obo/GAZ_00025533 -->

    <owl:NamedIndividual rdf:about="http://purl.obolibrary.org/obo/GAZ_00025533">
        <rdf:type rdf:resource="http://purl.obolibrary.org/obo/ENVO_00000004"/>
        <obo:RO_0001025 rdf:resource="http://purl.obolibrary.org/obo/GAZ_02000001"/>
        <obo:IAO_0000115>A district of the Mandalay Division in central Burma.</obo:IAO_0000115>
        <oboInOwl:hasOBONamespace>GAZ</oboInOwl:hasOBONamespace>
        <oboInOwl:id>GAZ:00025533</oboInOwl:id>
        <rdfs:label>Myingyan District</rdfs:label>
    </owl:NamedIndividual>
    


    <!-- http://purl.obolibrary.org/obo/GAZ_00025534 -->

    <owl:NamedIndividual rdf:about="http://purl.obolibrary.org/obo/GAZ_00025534">
        <rdf:type rdf:resource="http://purl.obolibrary.org/obo/ENVO_00000004"/>
        <obo:RO_0001025 rdf:resource="http://purl.obolibrary.org/obo/GAZ_02000001"/>
        <obo:IAO_0000115>A district of the Mandalay Division in central Burma.</obo:IAO_0000115>
        <oboInOwl:hasOBONamespace>GAZ</oboInOwl:hasOBONamespace>
        <oboInOwl:id>GAZ:00025534</oboInOwl:id>
        <rdfs:label>Nyaung-u District</rdfs:label>
    </owl:NamedIndividual>
    


    <!-- http://purl.obolibrary.org/obo/GAZ_00025535 -->

    <owl:NamedIndividual rdf:about="http://purl.obolibrary.org/obo/GAZ_00025535">
        <rdf:type rdf:resource="http://purl.obolibrary.org/obo/ENVO_00000004"/>
        <obo:RO_0001025 rdf:resource="http://purl.obolibrary.org/obo/GAZ_02000001"/>
        <obo:IAO_0000115>A district of the Mandalay Division in central Burma.</obo:IAO_0000115>
        <oboInOwl:hasOBONamespace>GAZ</oboInOwl:hasOBONamespace>
        <oboInOwl:id>GAZ:00025535</oboInOwl:id>
        <rdfs:label>Pyin-Oo-Lwin District</rdfs:label>
    </owl:NamedIndividual>
    


    <!-- http://purl.obolibrary.org/obo/GAZ_00025536 -->

    <owl:NamedIndividual rdf:about="http://purl.obolibrary.org/obo/GAZ_00025536">
        <rdf:type rdf:resource="http://purl.obolibrary.org/obo/ENVO_00000004"/>
        <obo:RO_0001025 rdf:resource="http://purl.obolibrary.org/obo/GAZ_02000001"/>
        <obo:IAO_0000115>A district of the Mandalay Division in central Burma.</obo:IAO_0000115>
        <oboInOwl:hasOBONamespace>GAZ</oboInOwl:hasOBONamespace>
        <oboInOwl:id>GAZ:00025536</oboInOwl:id>
        <rdfs:label>Yamethin District</rdfs:label>
    </owl:NamedIndividual>
    


    <!-- http://purl.obolibrary.org/obo/GAZ_00025537 -->

    <owl:NamedIndividual rdf:about="http://purl.obolibrary.org/obo/GAZ_00025537">
        <rdf:type rdf:resource="http://purl.obolibrary.org/obo/ENVO_00000004"/>
        <obo:RO_0001025 rdf:resource="http://purl.obolibrary.org/obo/GAZ_02000013"/>
        <obo:IAO_0000115>A district of the Chin State in Myanmar.</obo:IAO_0000115>
        <oboInOwl:hasOBONamespace>GAZ</oboInOwl:hasOBONamespace>
        <oboInOwl:id>GAZ:00025537</oboInOwl:id>
        <rdfs:label>Mindat District</rdfs:label>
    </owl:NamedIndividual>
    


    <!-- http://purl.obolibrary.org/obo/GAZ_00025538 -->

    <owl:NamedIndividual rdf:about="http://purl.obolibrary.org/obo/GAZ_00025538">
        <rdf:type rdf:resource="http://purl.obolibrary.org/obo/ENVO_00000004"/>
        <obo:RO_0001025 rdf:resource="http://purl.obolibrary.org/obo/GAZ_02000013"/>
        <obo:IAO_0000115>A district of the Chin State in Myanmar.</obo:IAO_0000115>
        <oboInOwl:hasOBONamespace>GAZ</oboInOwl:hasOBONamespace>
        <oboInOwl:id>GAZ:00025538</oboInOwl:id>
        <rdfs:label>Falam District</rdfs:label>
    </owl:NamedIndividual>
    


    <!-- http://purl.obolibrary.org/obo/GAZ_00025539 -->

    <owl:NamedIndividual rdf:about="http://purl.obolibrary.org/obo/GAZ_00025539">
        <rdf:type rdf:resource="http://purl.obolibrary.org/obo/ENVO_00000004"/>
        <obo:RO_0001025 rdf:resource="http://purl.obolibrary.org/obo/GAZ_02000012"/>
        <obo:IAO_0000115>A district of the Kachin State in northern Burma. The capital is Myitkyina.</obo:IAO_0000115>
        <oboInOwl:hasOBONamespace>GAZ</oboInOwl:hasOBONamespace>
        <oboInOwl:id>GAZ:00025539</oboInOwl:id>
        <rdfs:label>Myitkyina District</rdfs:label>
    </owl:NamedIndividual>
    


    <!-- http://purl.obolibrary.org/obo/GAZ_00025540 -->

    <owl:NamedIndividual rdf:about="http://purl.obolibrary.org/obo/GAZ_00025540">
        <rdf:type rdf:resource="http://purl.obolibrary.org/obo/ENVO_00000004"/>
        <obo:RO_0001025 rdf:resource="http://purl.obolibrary.org/obo/GAZ_02000012"/>
        <obo:IAO_0000115>A district of the Kachin State in northern Burma. The capital is Putao.</obo:IAO_0000115>
        <oboInOwl:hasOBONamespace>GAZ</oboInOwl:hasOBONamespace>
        <oboInOwl:id>GAZ:00025540</oboInOwl:id>
        <rdfs:label>Putao District</rdfs:label>
    </owl:NamedIndividual>
    


    <!-- http://purl.obolibrary.org/obo/GAZ_00025541 -->

    <owl:NamedIndividual rdf:about="http://purl.obolibrary.org/obo/GAZ_00025541">
        <rdf:type rdf:resource="http://purl.obolibrary.org/obo/ENVO_00000004"/>
        <obo:RO_0001025 rdf:resource="http://purl.obolibrary.org/obo/GAZ_02000012"/>
        <obo:IAO_0000115>A district of the Kachin State in northern Burma. The capital is Bhamo.</obo:IAO_0000115>
        <oboInOwl:hasOBONamespace>GAZ</oboInOwl:hasOBONamespace>
        <oboInOwl:id>GAZ:00025541</oboInOwl:id>
        <rdfs:label>Bhamo District</rdfs:label>
    </owl:NamedIndividual>
    


    <!-- http://purl.obolibrary.org/obo/GAZ_00025542 -->

    <owl:NamedIndividual rdf:about="http://purl.obolibrary.org/obo/GAZ_00025542">
        <rdf:type rdf:resource="http://purl.obolibrary.org/obo/ENVO_00000004"/>
        <obo:RO_0001025 rdf:resource="http://purl.obolibrary.org/obo/GAZ_02000011"/>
        <obo:IAO_0000115>A district of Kayah State.</obo:IAO_0000115>
        <oboInOwl:hasOBONamespace>GAZ</oboInOwl:hasOBONamespace>
        <oboInOwl:id>GAZ:00025542</oboInOwl:id>
        <rdfs:label>Loikaw District</rdfs:label>
    </owl:NamedIndividual>
    


    <!-- http://purl.obolibrary.org/obo/GAZ_00025543 -->

    <owl:NamedIndividual rdf:about="http://purl.obolibrary.org/obo/GAZ_00025543">
        <rdf:type rdf:resource="http://purl.obolibrary.org/obo/ENVO_00000004"/>
        <obo:RO_0001025 rdf:resource="http://purl.obolibrary.org/obo/GAZ_02000011"/>
        <obo:IAO_0000115>A district of Kayah State.</obo:IAO_0000115>
        <oboInOwl:hasOBONamespace>GAZ</oboInOwl:hasOBONamespace>
        <oboInOwl:id>GAZ:00025543</oboInOwl:id>
        <rdfs:label>Bawlakhe District</rdfs:label>
    </owl:NamedIndividual>
    


    <!-- http://purl.obolibrary.org/obo/GAZ_00025544 -->

    <owl:NamedIndividual rdf:about="http://purl.obolibrary.org/obo/GAZ_00025544">
        <rdf:type rdf:resource="http://purl.obolibrary.org/obo/ENVO_00000004"/>
        <obo:RO_0001025 rdf:resource="http://purl.obolibrary.org/obo/GAZ_02000009"/>
        <obo:IAO_0000115>A district of the Kayin State in Myanmar.</obo:IAO_0000115>
        <oboInOwl:hasOBONamespace>GAZ</oboInOwl:hasOBONamespace>
        <oboInOwl:id>GAZ:00025544</oboInOwl:id>
        <rdfs:label>Hpa-an District</rdfs:label>
    </owl:NamedIndividual>
    


    <!-- http://purl.obolibrary.org/obo/GAZ_00025545 -->

    <owl:NamedIndividual rdf:about="http://purl.obolibrary.org/obo/GAZ_00025545">
        <rdf:type rdf:resource="http://purl.obolibrary.org/obo/ENVO_00000004"/>
        <obo:RO_0001025 rdf:resource="http://purl.obolibrary.org/obo/GAZ_02000009"/>
        <obo:IAO_0000115>A district of the Kayin State in Myanmar.</obo:IAO_0000115>
        <oboInOwl:hasOBONamespace>GAZ</oboInOwl:hasOBONamespace>
        <oboInOwl:id>GAZ:00025545</oboInOwl:id>
        <rdfs:label>Kawkareik District</rdfs:label>
    </owl:NamedIndividual>
    


    <!-- http://purl.obolibrary.org/obo/GAZ_00025546 -->

    <owl:NamedIndividual rdf:about="http://purl.obolibrary.org/obo/GAZ_00025546">
        <rdf:type rdf:resource="http://purl.obolibrary.org/obo/ENVO_00000004"/>
        <obo:RO_0001025 rdf:resource="http://purl.obolibrary.org/obo/GAZ_02000009"/>
        <obo:IAO_0000115>A district of the Kayin State in Myanmar.</obo:IAO_0000115>
        <oboInOwl:hasOBONamespace>GAZ</oboInOwl:hasOBONamespace>
        <oboInOwl:id>GAZ:00025546</oboInOwl:id>
        <rdfs:label>Myawadi District</rdfs:label>
    </owl:NamedIndividual>
    


    <!-- http://purl.obolibrary.org/obo/GAZ_00025547 -->

    <owl:NamedIndividual rdf:about="http://purl.obolibrary.org/obo/GAZ_00025547">
        <rdf:type rdf:resource="http://purl.obolibrary.org/obo/ENVO_00000004"/>
        <obo:RO_0001025 rdf:resource="http://purl.obolibrary.org/obo/GAZ_02000008"/>
        <obo:IAO_0000115>A district of the Mon State in Myanmar. The capital is Mawlamyine town.</obo:IAO_0000115>
        <oboInOwl:hasOBONamespace>GAZ</oboInOwl:hasOBONamespace>
        <oboInOwl:id>GAZ:00025547</oboInOwl:id>
        <rdfs:label>Mawlamyine District</rdfs:label>
    </owl:NamedIndividual>
    


    <!-- http://purl.obolibrary.org/obo/GAZ_00025548 -->

    <owl:NamedIndividual rdf:about="http://purl.obolibrary.org/obo/GAZ_00025548">
        <rdf:type rdf:resource="http://purl.obolibrary.org/obo/ENVO_00000004"/>
        <obo:RO_0001025 rdf:resource="http://purl.obolibrary.org/obo/GAZ_02000008"/>
        <obo:IAO_0000115>A district of the Mon State in Myanmar. The capital is Thaton town.</obo:IAO_0000115>
        <oboInOwl:hasOBONamespace>GAZ</oboInOwl:hasOBONamespace>
        <oboInOwl:id>GAZ:00025548</oboInOwl:id>
        <rdfs:label>Thaton District</rdfs:label>
    </owl:NamedIndividual>
    


    <!-- http://purl.obolibrary.org/obo/GAZ_00025549 -->

    <owl:NamedIndividual rdf:about="http://purl.obolibrary.org/obo/GAZ_00025549">
        <obo:RO_0001025 rdf:resource="http://purl.obolibrary.org/obo/GAZ_02000010"/>
        <oboInOwl:hasOBONamespace>GAZ</oboInOwl:hasOBONamespace>
        <oboInOwl:id>GAZ:00025549</oboInOwl:id>
        <rdfs:label>Buthidaung District</rdfs:label>
    </owl:NamedIndividual>
    


    <!-- http://purl.obolibrary.org/obo/GAZ_00025550 -->

    <owl:NamedIndividual rdf:about="http://purl.obolibrary.org/obo/GAZ_00025550">
        <rdf:type rdf:resource="http://purl.obolibrary.org/obo/ENVO_00000004"/>
        <obo:RO_0001025 rdf:resource="http://purl.obolibrary.org/obo/GAZ_02000010"/>
        <obo:IAO_0000115>A district of the Rakhine State in western Myanmar. The capital is Kyaukpyu.</obo:IAO_0000115>
        <oboInOwl:hasOBONamespace>GAZ</oboInOwl:hasOBONamespace>
        <oboInOwl:id>GAZ:00025550</oboInOwl:id>
        <rdfs:label>Kyaunkpyu District</rdfs:label>
    </owl:NamedIndividual>
    


    <!-- http://purl.obolibrary.org/obo/GAZ_00025551 -->

    <owl:NamedIndividual rdf:about="http://purl.obolibrary.org/obo/GAZ_00025551">
        <rdf:type rdf:resource="http://purl.obolibrary.org/obo/ENVO_00000004"/>
        <obo:RO_0001025 rdf:resource="http://purl.obolibrary.org/obo/GAZ_02000010"/>
        <obo:IAO_0000115>A district of the Rakhine State in western Myanmar. The capital lies at Sittwe.</obo:IAO_0000115>
        <oboInOwl:hasOBONamespace>GAZ</oboInOwl:hasOBONamespace>
        <oboInOwl:id>GAZ:00025551</oboInOwl:id>
        <rdfs:label>Maungdaw District</rdfs:label>
    </owl:NamedIndividual>
    


    <!-- http://purl.obolibrary.org/obo/GAZ_00025552 -->

    <owl:NamedIndividual rdf:about="http://purl.obolibrary.org/obo/GAZ_00025552">
        <rdf:type rdf:resource="http://purl.obolibrary.org/obo/ENVO_00000004"/>
        <obo:RO_0001025 rdf:resource="http://purl.obolibrary.org/obo/GAZ_02000010"/>
        <obo:IAO_0000115>A district of the Rakhine State in western Myanmar. The capital is Sittwe.</obo:IAO_0000115>
        <oboInOwl:hasOBONamespace>GAZ</oboInOwl:hasOBONamespace>
        <oboInOwl:id>GAZ:00025552</oboInOwl:id>
        <rdfs:label>Sittwe District</rdfs:label>
    </owl:NamedIndividual>
    


    <!-- http://purl.obolibrary.org/obo/GAZ_00025553 -->

    <owl:NamedIndividual rdf:about="http://purl.obolibrary.org/obo/GAZ_00025553">
        <rdf:type rdf:resource="http://purl.obolibrary.org/obo/ENVO_00000004"/>
        <obo:RO_0001025 rdf:resource="http://purl.obolibrary.org/obo/GAZ_02000010"/>
        <obo:IAO_0000115>A district of the Rakhine State in western Myanmar. The capital lies at Thandwe.</obo:IAO_0000115>
        <oboInOwl:hasOBONamespace>GAZ</oboInOwl:hasOBONamespace>
        <oboInOwl:id>GAZ:00025553</oboInOwl:id>
        <rdfs:label>Thandwe District</rdfs:label>
    </owl:NamedIndividual>
    


    <!-- http://purl.obolibrary.org/obo/GAZ_00025554 -->

    <owl:NamedIndividual rdf:about="http://purl.obolibrary.org/obo/GAZ_00025554">
        <rdf:type rdf:resource="http://purl.obolibrary.org/obo/ENVO_00000004"/>
        <obo:RO_0001025 rdf:resource="http://purl.obolibrary.org/obo/GAZ_02000007"/>
        <obo:IAO_0000115>A district of the Shan State in Myanmar.</obo:IAO_0000115>
        <oboInOwl:hasOBONamespace>GAZ</oboInOwl:hasOBONamespace>
        <oboInOwl:id>GAZ:00025554</oboInOwl:id>
        <rdfs:label>Kengtung District</rdfs:label>
    </owl:NamedIndividual>
    


    <!-- http://purl.obolibrary.org/obo/GAZ_00025555 -->

    <owl:NamedIndividual rdf:about="http://purl.obolibrary.org/obo/GAZ_00025555">
        <rdf:type rdf:resource="http://purl.obolibrary.org/obo/ENVO_00000004"/>
        <obo:RO_0001025 rdf:resource="http://purl.obolibrary.org/obo/GAZ_02000007"/>
        <obo:IAO_0000115>A district of the Shan State in Myanmar.</obo:IAO_0000115>
        <oboInOwl:hasOBONamespace>GAZ</oboInOwl:hasOBONamespace>
        <oboInOwl:id>GAZ:00025555</oboInOwl:id>
        <rdfs:label>Kunlong District</rdfs:label>
    </owl:NamedIndividual>
    


    <!-- http://purl.obolibrary.org/obo/GAZ_00025556 -->

    <owl:NamedIndividual rdf:about="http://purl.obolibrary.org/obo/GAZ_00025556">
        <rdf:type rdf:resource="http://purl.obolibrary.org/obo/ENVO_00000004"/>
        <obo:RO_0001025 rdf:resource="http://purl.obolibrary.org/obo/GAZ_02000007"/>
        <obo:IAO_0000115>A district of the Shan State in Myanmar.</obo:IAO_0000115>
        <oboInOwl:hasOBONamespace>GAZ</oboInOwl:hasOBONamespace>
        <oboInOwl:id>GAZ:00025556</oboInOwl:id>
        <rdfs:label>Kyaukme District</rdfs:label>
    </owl:NamedIndividual>
    


    <!-- http://purl.obolibrary.org/obo/GAZ_00025557 -->

    <owl:NamedIndividual rdf:about="http://purl.obolibrary.org/obo/GAZ_00025557">
        <rdf:type rdf:resource="http://purl.obolibrary.org/obo/ENVO_00000004"/>
        <obo:RO_0001025 rdf:resource="http://purl.obolibrary.org/obo/GAZ_02000007"/>
        <obo:IAO_0000115>A district of the Shan State in Myanmar.</obo:IAO_0000115>
        <oboInOwl:hasOBONamespace>GAZ</oboInOwl:hasOBONamespace>
        <oboInOwl:id>GAZ:00025557</oboInOwl:id>
        <rdfs:label>Lashio District</rdfs:label>
    </owl:NamedIndividual>
    


    <!-- http://purl.obolibrary.org/obo/GAZ_00025558 -->

    <owl:NamedIndividual rdf:about="http://purl.obolibrary.org/obo/GAZ_00025558">
        <rdf:type rdf:resource="http://purl.obolibrary.org/obo/ENVO_00000004"/>
        <obo:RO_0001025 rdf:resource="http://purl.obolibrary.org/obo/GAZ_02000007"/>
        <obo:IAO_0000115>A district of the Shan State in Myanmar.</obo:IAO_0000115>
        <oboInOwl:hasOBONamespace>GAZ</oboInOwl:hasOBONamespace>
        <oboInOwl:id>GAZ:00025558</oboInOwl:id>
        <rdfs:label>Laukkaing District</rdfs:label>
    </owl:NamedIndividual>
    


    <!-- http://purl.obolibrary.org/obo/GAZ_00025559 -->

    <owl:NamedIndividual rdf:about="http://purl.obolibrary.org/obo/GAZ_00025559">
        <rdf:type rdf:resource="http://purl.obolibrary.org/obo/ENVO_00000004"/>
        <obo:RO_0001025 rdf:resource="http://purl.obolibrary.org/obo/GAZ_02000007"/>
        <obo:IAO_0000115>A district of the Shan State in Myanmar.</obo:IAO_0000115>
        <oboInOwl:hasOBONamespace>GAZ</oboInOwl:hasOBONamespace>
        <oboInOwl:id>GAZ:00025559</oboInOwl:id>
        <rdfs:label>Loilen District</rdfs:label>
    </owl:NamedIndividual>
    


    <!-- http://purl.obolibrary.org/obo/GAZ_00025560 -->

    <owl:NamedIndividual rdf:about="http://purl.obolibrary.org/obo/GAZ_00025560">
        <rdf:type rdf:resource="http://purl.obolibrary.org/obo/ENVO_00000004"/>
        <obo:RO_0001025 rdf:resource="http://purl.obolibrary.org/obo/GAZ_02000007"/>
        <obo:IAO_0000115>A district of the Shan State in Myanmar.</obo:IAO_0000115>
        <oboInOwl:hasOBONamespace>GAZ</oboInOwl:hasOBONamespace>
        <oboInOwl:id>GAZ:00025560</oboInOwl:id>
        <rdfs:label>Mong-Hpayak District</rdfs:label>
    </owl:NamedIndividual>
    


    <!-- http://purl.obolibrary.org/obo/GAZ_00025561 -->

    <owl:NamedIndividual rdf:about="http://purl.obolibrary.org/obo/GAZ_00025561">
        <rdf:type rdf:resource="http://purl.obolibrary.org/obo/ENVO_00000004"/>
        <obo:RO_0001025 rdf:resource="http://purl.obolibrary.org/obo/GAZ_02000007"/>
        <obo:IAO_0000115>A district of the Shan State in Myanmar.</obo:IAO_0000115>
        <oboInOwl:hasOBONamespace>GAZ</oboInOwl:hasOBONamespace>
        <oboInOwl:id>GAZ:00025561</oboInOwl:id>
        <rdfs:label>Mong Hsat District</rdfs:label>
    </owl:NamedIndividual>
    


    <!-- http://purl.obolibrary.org/obo/GAZ_00025562 -->

    <owl:NamedIndividual rdf:about="http://purl.obolibrary.org/obo/GAZ_00025562">
        <rdf:type rdf:resource="http://purl.obolibrary.org/obo/ENVO_00000004"/>
        <obo:RO_0001025 rdf:resource="http://purl.obolibrary.org/obo/GAZ_02000007"/>
        <obo:IAO_0000115>A district of the Shan State in Myanmar.</obo:IAO_0000115>
        <oboInOwl:hasOBONamespace>GAZ</oboInOwl:hasOBONamespace>
        <oboInOwl:id>GAZ:00025562</oboInOwl:id>
        <rdfs:label>Mu Se District</rdfs:label>
    </owl:NamedIndividual>
    


    <!-- http://purl.obolibrary.org/obo/GAZ_00025563 -->

    <owl:NamedIndividual rdf:about="http://purl.obolibrary.org/obo/GAZ_00025563">
        <rdf:type rdf:resource="http://purl.obolibrary.org/obo/ENVO_00000004"/>
        <obo:RO_0001025 rdf:resource="http://purl.obolibrary.org/obo/GAZ_02000007"/>
        <obo:IAO_0000115>A district of the Shan State in Myanmar.</obo:IAO_0000115>
        <oboInOwl:hasOBONamespace>GAZ</oboInOwl:hasOBONamespace>
        <oboInOwl:id>GAZ:00025563</oboInOwl:id>
        <rdfs:label>Tachileik District</rdfs:label>
    </owl:NamedIndividual>
    


    <!-- http://purl.obolibrary.org/obo/GAZ_00025564 -->

    <owl:NamedIndividual rdf:about="http://purl.obolibrary.org/obo/GAZ_00025564">
        <rdf:type rdf:resource="http://purl.obolibrary.org/obo/ENVO_00000004"/>
        <obo:RO_0001025 rdf:resource="http://purl.obolibrary.org/obo/GAZ_02000007"/>
        <obo:IAO_0000115>A district of Shan State in Burma. The principal town is Taunggyi.</obo:IAO_0000115>
        <oboInOwl:hasOBONamespace>GAZ</oboInOwl:hasOBONamespace>
        <oboInOwl:id>GAZ:00025564</oboInOwl:id>
        <rdfs:label>Taunggyi District</rdfs:label>
    </owl:NamedIndividual>
    


    <!-- http://purl.obolibrary.org/obo/GAZ_00043398 -->

    <owl:NamedIndividual rdf:about="http://purl.obolibrary.org/obo/GAZ_00043398">
        <obo:RO_0001025 rdf:resource="http://purl.obolibrary.org/obo/GAZ_00017493"/>
        <obo:IAO_0000115>An island in the Mergui Archipelago, Burma.</obo:IAO_0000115>
        <oboInOwl:hasOBONamespace>GAZ</oboInOwl:hasOBONamespace>
        <oboInOwl:id>GAZ:00043398</oboInOwl:id>
        <rdfs:label>Kadan Kyun</rdfs:label>
    </owl:NamedIndividual>
    


    <!-- http://purl.obolibrary.org/obo/GAZ_00043399 -->

    <owl:NamedIndividual rdf:about="http://purl.obolibrary.org/obo/GAZ_00043399">
        <obo:RO_0001025 rdf:resource="http://purl.obolibrary.org/obo/GAZ_00017493"/>
        <oboInOwl:hasOBONamespace>GAZ</oboInOwl:hasOBONamespace>
        <oboInOwl:id>GAZ:00043399</oboInOwl:id>
        <rdfs:label>Parker Island</rdfs:label>
    </owl:NamedIndividual>
    


    <!-- http://purl.obolibrary.org/obo/GAZ_00043400 -->

    <owl:NamedIndividual rdf:about="http://purl.obolibrary.org/obo/GAZ_00043400">
        <obo:RO_0001025 rdf:resource="http://purl.obolibrary.org/obo/GAZ_00017493"/>
        <obo:IAO_0000115>An island in the Mergui Archipelago, Burma (Myanmar).</obo:IAO_0000115>
        <oboInOwl:hasOBONamespace>GAZ</oboInOwl:hasOBONamespace>
        <oboInOwl:id>GAZ:00043400</oboInOwl:id>
        <rdfs:label>Mali Kyun</rdfs:label>
    </owl:NamedIndividual>
    


    <!-- http://purl.obolibrary.org/obo/GAZ_00043401 -->

    <owl:NamedIndividual rdf:about="http://purl.obolibrary.org/obo/GAZ_00043401">
        <obo:RO_0001025 rdf:resource="http://purl.obolibrary.org/obo/GAZ_00017493"/>
        <oboInOwl:hasOBONamespace>GAZ</oboInOwl:hasOBONamespace>
        <oboInOwl:id>GAZ:00043401</oboInOwl:id>
        <rdfs:label>Sabi Kyun</rdfs:label>
    </owl:NamedIndividual>
    


    <!-- http://purl.obolibrary.org/obo/GAZ_00043402 -->

    <owl:NamedIndividual rdf:about="http://purl.obolibrary.org/obo/GAZ_00043402">
        <obo:RO_0001025 rdf:resource="http://purl.obolibrary.org/obo/GAZ_00017493"/>
        <oboInOwl:hasOBONamespace>GAZ</oboInOwl:hasOBONamespace>
        <oboInOwl:id>GAZ:00043402</oboInOwl:id>
        <rdfs:label>Thamihla Kyun</rdfs:label>
    </owl:NamedIndividual>
    


    <!-- http://purl.obolibrary.org/obo/GAZ_00043403 -->

    <owl:NamedIndividual rdf:about="http://purl.obolibrary.org/obo/GAZ_00043403">
        <obo:RO_0001025 rdf:resource="http://purl.obolibrary.org/obo/GAZ_00017493"/>
        <oboInOwl:hasOBONamespace>GAZ</oboInOwl:hasOBONamespace>
        <oboInOwl:id>GAZ:00043403</oboInOwl:id>
        <rdfs:label>Maingy Island</rdfs:label>
    </owl:NamedIndividual>
    


    <!-- http://purl.obolibrary.org/obo/GAZ_00043404 -->

    <owl:NamedIndividual rdf:about="http://purl.obolibrary.org/obo/GAZ_00043404">
        <obo:RO_0001025 rdf:resource="http://purl.obolibrary.org/obo/GAZ_00017493"/>
        <oboInOwl:hasOBONamespace>GAZ</oboInOwl:hasOBONamespace>
        <oboInOwl:id>GAZ:00043404</oboInOwl:id>
        <rdfs:label>Mali Nge Island</rdfs:label>
    </owl:NamedIndividual>
    


    <!-- http://purl.obolibrary.org/obo/GAZ_00043405 -->

    <owl:NamedIndividual rdf:about="http://purl.obolibrary.org/obo/GAZ_00043405">
        <obo:RO_0001025 rdf:resource="http://purl.obolibrary.org/obo/GAZ_00017493"/>
        <obo:IAO_0000115>An island in the Mergui Archipelago, Burma (Myanmar).</obo:IAO_0000115>
        <oboInOwl:hasOBONamespace>GAZ</oboInOwl:hasOBONamespace>
        <oboInOwl:id>GAZ:00043405</oboInOwl:id>
        <rdfs:label>Daung Kyun</rdfs:label>
    </owl:NamedIndividual>
    


    <!-- http://purl.obolibrary.org/obo/GAZ_00043406 -->

    <owl:NamedIndividual rdf:about="http://purl.obolibrary.org/obo/GAZ_00043406">
        <obo:RO_0001025 rdf:resource="http://purl.obolibrary.org/obo/GAZ_00017493"/>
        <obo:IAO_0000115>An island in the Mergui Archipelago, Burma (Myanmar).</obo:IAO_0000115>
        <oboInOwl:hasOBONamespace>GAZ</oboInOwl:hasOBONamespace>
        <oboInOwl:id>GAZ:00043406</oboInOwl:id>
        <rdfs:label>Saganthit Kyun</rdfs:label>
    </owl:NamedIndividual>
    


    <!-- http://purl.obolibrary.org/obo/GAZ_00043407 -->

    <owl:NamedIndividual rdf:about="http://purl.obolibrary.org/obo/GAZ_00043407">
        <obo:RO_0001025 rdf:resource="http://purl.obolibrary.org/obo/GAZ_00017493"/>
        <oboInOwl:hasOBONamespace>GAZ</oboInOwl:hasOBONamespace>
        <oboInOwl:id>GAZ:00043407</oboInOwl:id>
        <rdfs:label>Lampi Island</rdfs:label>
    </owl:NamedIndividual>
    


    <!-- http://purl.obolibrary.org/obo/GAZ_00043408 -->

    <owl:NamedIndividual rdf:about="http://purl.obolibrary.org/obo/GAZ_00043408">
        <obo:RO_0001025 rdf:resource="http://purl.obolibrary.org/obo/GAZ_00017493"/>
        <oboInOwl:hasOBONamespace>GAZ</oboInOwl:hasOBONamespace>
        <oboInOwl:id>GAZ:00043408</oboInOwl:id>
        <rdfs:label>Ale-Man Kyun</rdfs:label>
    </owl:NamedIndividual>
    


    <!-- http://purl.obolibrary.org/obo/GAZ_00043409 -->

    <owl:NamedIndividual rdf:about="http://purl.obolibrary.org/obo/GAZ_00043409">
        <obo:RO_0001025 rdf:resource="http://purl.obolibrary.org/obo/GAZ_00017493"/>
        <oboInOwl:hasOBONamespace>GAZ</oboInOwl:hasOBONamespace>
        <oboInOwl:id>GAZ:00043409</oboInOwl:id>
        <rdfs:label>Paulu Bada</rdfs:label>
    </owl:NamedIndividual>
    


    <!-- http://purl.obolibrary.org/obo/GAZ_00043410 -->

    <owl:NamedIndividual rdf:about="http://purl.obolibrary.org/obo/GAZ_00043410">
        <obo:RO_0001025 rdf:resource="http://purl.obolibrary.org/obo/GAZ_00017493"/>
        <obo:IAO_0000115>An island in the Mergui Archipelago, Burma.</obo:IAO_0000115>
        <oboInOwl:hasOBONamespace>GAZ</oboInOwl:hasOBONamespace>
        <oboInOwl:id>GAZ:00043410</oboInOwl:id>
        <rdfs:label>Kanmaw Kyun</rdfs:label>
    </owl:NamedIndividual>
    


    <!-- http://purl.obolibrary.org/obo/GAZ_00043411 -->

    <owl:NamedIndividual rdf:about="http://purl.obolibrary.org/obo/GAZ_00043411">
        <obo:RO_0001025 rdf:resource="http://purl.obolibrary.org/obo/GAZ_00017493"/>
        <oboInOwl:hasOBONamespace>GAZ</oboInOwl:hasOBONamespace>
        <oboInOwl:id>GAZ:00043411</oboInOwl:id>
        <rdfs:label>Kau-Ye Kyun</rdfs:label>
    </owl:NamedIndividual>
    


    <!-- http://purl.obolibrary.org/obo/GAZ_00043412 -->

    <owl:NamedIndividual rdf:about="http://purl.obolibrary.org/obo/GAZ_00043412">
        <obo:RO_0001025 rdf:resource="http://purl.obolibrary.org/obo/GAZ_00017493"/>
        <oboInOwl:hasOBONamespace>GAZ</oboInOwl:hasOBONamespace>
        <oboInOwl:id>GAZ:00043412</oboInOwl:id>
        <rdfs:label>Than Kyun</rdfs:label>
    </owl:NamedIndividual>
    


    <!-- http://purl.obolibrary.org/obo/GAZ_00043413 -->

    <owl:NamedIndividual rdf:about="http://purl.obolibrary.org/obo/GAZ_00043413">
        <obo:RO_0001025 rdf:resource="http://purl.obolibrary.org/obo/GAZ_00017493"/>
        <oboInOwl:hasOBONamespace>GAZ</oboInOwl:hasOBONamespace>
        <oboInOwl:id>GAZ:00043413</oboInOwl:id>
        <rdfs:label>Zadetkale Kyun</rdfs:label>
    </owl:NamedIndividual>
    


    <!-- http://purl.obolibrary.org/obo/GAZ_00043414 -->

    <owl:NamedIndividual rdf:about="http://purl.obolibrary.org/obo/GAZ_00043414">
        <obo:RO_0001025 rdf:resource="http://purl.obolibrary.org/obo/GAZ_00017493"/>
        <oboInOwl:hasOBONamespace>GAZ</oboInOwl:hasOBONamespace>
        <oboInOwl:id>GAZ:00043414</oboInOwl:id>
        <rdfs:label>Hastings Island</rdfs:label>
    </owl:NamedIndividual>
    


    <!-- http://purl.obolibrary.org/obo/GAZ_00043415 -->

    <owl:NamedIndividual rdf:about="http://purl.obolibrary.org/obo/GAZ_00043415">
        <obo:RO_0001025 rdf:resource="http://purl.obolibrary.org/obo/GAZ_00017493"/>
        <oboInOwl:hasOBONamespace>GAZ</oboInOwl:hasOBONamespace>
        <oboInOwl:id>GAZ:00043415</oboInOwl:id>
        <rdfs:label>Zadetkyl Kyun</rdfs:label>
    </owl:NamedIndividual>
    


    <!-- http://purl.obolibrary.org/obo/GAZ_00043416 -->

    <owl:NamedIndividual rdf:about="http://purl.obolibrary.org/obo/GAZ_00043416">
        <obo:RO_0001025 rdf:resource="http://purl.obolibrary.org/obo/GAZ_00017493"/>
        <oboInOwl:hasOBONamespace>GAZ</oboInOwl:hasOBONamespace>
        <oboInOwl:id>GAZ:00043416</oboInOwl:id>
        <rdfs:label>Owen Island</rdfs:label>
    </owl:NamedIndividual>
    


    <!-- http://purl.obolibrary.org/obo/GAZ_00043417 -->

    <owl:NamedIndividual rdf:about="http://purl.obolibrary.org/obo/GAZ_00043417">
        <obo:RO_0001025 rdf:resource="http://purl.obolibrary.org/obo/GAZ_00017493"/>
        <oboInOwl:hasOBONamespace>GAZ</oboInOwl:hasOBONamespace>
        <oboInOwl:id>GAZ:00043417</oboInOwl:id>
        <rdfs:label>Christie Island</rdfs:label>
    </owl:NamedIndividual>
    


    <!-- http://purl.obolibrary.org/obo/GAZ_00043418 -->

    <owl:NamedIndividual rdf:about="http://purl.obolibrary.org/obo/GAZ_00043418">
        <obo:RO_0001025 rdf:resource="http://purl.obolibrary.org/obo/GAZ_00017493"/>
        <oboInOwl:hasOBONamespace>GAZ</oboInOwl:hasOBONamespace>
        <oboInOwl:id>GAZ:00043418</oboInOwl:id>
        <rdfs:label>North Twin Island</rdfs:label>
    </owl:NamedIndividual>
    


    <!-- http://purl.obolibrary.org/obo/GAZ_00043419 -->

    <owl:NamedIndividual rdf:about="http://purl.obolibrary.org/obo/GAZ_00043419">
        <obo:RO_0001025 rdf:resource="http://purl.obolibrary.org/obo/GAZ_00017493"/>
        <oboInOwl:hasOBONamespace>GAZ</oboInOwl:hasOBONamespace>
        <oboInOwl:id>GAZ:00043419</oboInOwl:id>
        <rdfs:label>MacLeod Island</rdfs:label>
    </owl:NamedIndividual>
    


    <!-- http://purl.obolibrary.org/obo/GAZ_00043420 -->

    <owl:NamedIndividual rdf:about="http://purl.obolibrary.org/obo/GAZ_00043420">
        <obo:RO_0001025 rdf:resource="http://purl.obolibrary.org/obo/GAZ_00017493"/>
        <oboInOwl:hasOBONamespace>GAZ</oboInOwl:hasOBONamespace>
        <oboInOwl:id>GAZ:00043420</oboInOwl:id>
        <rdfs:label>McCarthy Island</rdfs:label>
    </owl:NamedIndividual>
    


    <!-- http://purl.obolibrary.org/obo/GAZ_00043421 -->

    <owl:NamedIndividual rdf:about="http://purl.obolibrary.org/obo/GAZ_00043421">
        <obo:RO_0001025 rdf:resource="http://purl.obolibrary.org/obo/GAZ_00017493"/>
        <oboInOwl:hasOBONamespace>GAZ</oboInOwl:hasOBONamespace>
        <oboInOwl:id>GAZ:00043421</oboInOwl:id>
        <rdfs:label>Clara Island</rdfs:label>
    </owl:NamedIndividual>
    


    <!-- http://purl.obolibrary.org/obo/GAZ_00043422 -->

    <owl:NamedIndividual rdf:about="http://purl.obolibrary.org/obo/GAZ_00043422">
        <obo:RO_0001025 rdf:resource="http://purl.obolibrary.org/obo/GAZ_00017493"/>
        <oboInOwl:hasOBONamespace>GAZ</oboInOwl:hasOBONamespace>
        <oboInOwl:id>GAZ:00043422</oboInOwl:id>
        <rdfs:label>Stewart Island</rdfs:label>
    </owl:NamedIndividual>
    


    <!-- http://purl.obolibrary.org/obo/GAZ_00043423 -->

    <owl:NamedIndividual rdf:about="http://purl.obolibrary.org/obo/GAZ_00043423">
        <obo:RO_0001025 rdf:resource="http://purl.obolibrary.org/obo/GAZ_00017493"/>
        <oboInOwl:hasOBONamespace>GAZ</oboInOwl:hasOBONamespace>
        <oboInOwl:id>GAZ:00043423</oboInOwl:id>
        <rdfs:label>South Twin Island</rdfs:label>
    </owl:NamedIndividual>
    


    <!-- http://purl.obolibrary.org/obo/GAZ_00043424 -->

    <owl:NamedIndividual rdf:about="http://purl.obolibrary.org/obo/GAZ_00043424">
        <obo:RO_0001025 rdf:resource="http://purl.obolibrary.org/obo/GAZ_00017493"/>
        <oboInOwl:hasOBONamespace>GAZ</oboInOwl:hasOBONamespace>
        <oboInOwl:id>GAZ:00043424</oboInOwl:id>
        <rdfs:label>Lord Loughborough Island</rdfs:label>
    </owl:NamedIndividual>
    


    <!-- http://purl.obolibrary.org/obo/GAZ_00043425 -->

    <owl:NamedIndividual rdf:about="http://purl.obolibrary.org/obo/GAZ_00043425">
        <obo:RO_0001025 rdf:resource="http://purl.obolibrary.org/obo/GAZ_00017493"/>
        <oboInOwl:hasOBONamespace>GAZ</oboInOwl:hasOBONamespace>
        <oboInOwl:id>GAZ:00043425</oboInOwl:id>
        <rdfs:label>Lloyds Island</rdfs:label>
    </owl:NamedIndividual>
    


    <!-- http://purl.obolibrary.org/obo/GAZ_00043426 -->

    <owl:NamedIndividual rdf:about="http://purl.obolibrary.org/obo/GAZ_00043426">
        <obo:RO_0001025 rdf:resource="http://purl.obolibrary.org/obo/GAZ_00017493"/>
        <oboInOwl:hasOBONamespace>GAZ</oboInOwl:hasOBONamespace>
        <oboInOwl:id>GAZ:00043426</oboInOwl:id>
        <rdfs:label>Kunthi Kyun</rdfs:label>
    </owl:NamedIndividual>
    


    <!-- http://purl.obolibrary.org/obo/GAZ_00043427 -->

    <owl:NamedIndividual rdf:about="http://purl.obolibrary.org/obo/GAZ_00043427">
        <obo:RO_0001025 rdf:resource="http://purl.obolibrary.org/obo/GAZ_00017493"/>
        <oboInOwl:hasOBONamespace>GAZ</oboInOwl:hasOBONamespace>
        <oboInOwl:id>GAZ:00043427</oboInOwl:id>
        <rdfs:label>Sir J. Malcolm Island</rdfs:label>
    </owl:NamedIndividual>
    


    <!-- http://purl.obolibrary.org/obo/GAZ_00043428 -->

    <owl:NamedIndividual rdf:about="http://purl.obolibrary.org/obo/GAZ_00043428">
        <obo:RO_0001025 rdf:resource="http://purl.obolibrary.org/obo/GAZ_00017493"/>
        <oboInOwl:hasOBONamespace>GAZ</oboInOwl:hasOBONamespace>
        <oboInOwl:id>GAZ:00043428</oboInOwl:id>
        <rdfs:label>Eliza Island</rdfs:label>
    </owl:NamedIndividual>
    


    <!-- http://purl.obolibrary.org/obo/GAZ_00043429 -->

    <owl:NamedIndividual rdf:about="http://purl.obolibrary.org/obo/GAZ_00043429">
        <obo:RO_0001025 rdf:resource="http://purl.obolibrary.org/obo/GAZ_00017493"/>
        <oboInOwl:hasOBONamespace>GAZ</oboInOwl:hasOBONamespace>
        <oboInOwl:id>GAZ:00043429</oboInOwl:id>
        <rdfs:label>Seargent Island</rdfs:label>
    </owl:NamedIndividual>
    


    <!-- http://purl.obolibrary.org/obo/GAZ_00043430 -->

    <owl:NamedIndividual rdf:about="http://purl.obolibrary.org/obo/GAZ_00043430">
        <obo:RO_0001025 rdf:resource="http://purl.obolibrary.org/obo/GAZ_00017493"/>
        <oboInOwl:hasOBONamespace>GAZ</oboInOwl:hasOBONamespace>
        <oboInOwl:id>GAZ:00043430</oboInOwl:id>
        <rdfs:label>Great West Torres Islands</rdfs:label>
    </owl:NamedIndividual>
    


    <!-- http://purl.obolibrary.org/obo/GAZ_00043431 -->

    <owl:NamedIndividual rdf:about="http://purl.obolibrary.org/obo/GAZ_00043431">
        <obo:RO_0001025 rdf:resource="http://purl.obolibrary.org/obo/GAZ_00017493"/>
        <oboInOwl:hasOBONamespace>GAZ</oboInOwl:hasOBONamespace>
        <oboInOwl:id>GAZ:00043431</oboInOwl:id>
        <rdfs:label>Western Island</rdfs:label>
    </owl:NamedIndividual>
    


    <!-- http://purl.obolibrary.org/obo/GAZ_00043432 -->

    <owl:NamedIndividual rdf:about="http://purl.obolibrary.org/obo/GAZ_00043432">
        <obo:RO_0001025 rdf:resource="http://purl.obolibrary.org/obo/GAZ_00017493"/>
        <obo:IAO_0000115>An island in the Mergui Archipelago, Burma (Myanmar).</obo:IAO_0000115>
        <oboInOwl:hasOBONamespace>GAZ</oboInOwl:hasOBONamespace>
        <oboInOwl:id>GAZ:00043432</oboInOwl:id>
        <rdfs:label>Letsok-aw Kyun</rdfs:label>
    </owl:NamedIndividual>
    


    <!-- http://purl.obolibrary.org/obo/GAZ_00043433 -->

    <owl:NamedIndividual rdf:about="http://purl.obolibrary.org/obo/GAZ_00043433">
        <obo:RO_0001025 rdf:resource="http://purl.obolibrary.org/obo/GAZ_00017493"/>
        <oboInOwl:hasOBONamespace>GAZ</oboInOwl:hasOBONamespace>
        <oboInOwl:id>GAZ:00043433</oboInOwl:id>
        <rdfs:label>Mackenzie Island</rdfs:label>
    </owl:NamedIndividual>
    


    <!-- http://purl.obolibrary.org/obo/GAZ_00043434 -->

    <owl:NamedIndividual rdf:about="http://purl.obolibrary.org/obo/GAZ_00043434">
        <obo:RO_0001025 rdf:resource="http://purl.obolibrary.org/obo/GAZ_00017493"/>
        <oboInOwl:hasOBONamespace>GAZ</oboInOwl:hasOBONamespace>
        <oboInOwl:id>GAZ:00043434</oboInOwl:id>
        <rdfs:label>Chester Island</rdfs:label>
    </owl:NamedIndividual>
    


    <!-- http://purl.obolibrary.org/obo/GAZ_00043435 -->

    <owl:NamedIndividual rdf:about="http://purl.obolibrary.org/obo/GAZ_00043435">
        <obo:RO_0001025 rdf:resource="http://purl.obolibrary.org/obo/GAZ_00017493"/>
        <obo:IAO_0000115>An island in the Mergui Archipelago, Burma (Myanmar).</obo:IAO_0000115>
        <oboInOwl:hasOBONamespace>GAZ</oboInOwl:hasOBONamespace>
        <oboInOwl:id>GAZ:00043435</oboInOwl:id>
        <rdfs:label>Bentinck Kyun</rdfs:label>
    </owl:NamedIndividual>
    


    <!-- http://purl.obolibrary.org/obo/GAZ_00043436 -->

    <owl:NamedIndividual rdf:about="http://purl.obolibrary.org/obo/GAZ_00043436">
        <obo:RO_0001025 rdf:resource="http://purl.obolibrary.org/obo/GAZ_00017493"/>
        <oboInOwl:hasOBONamespace>GAZ</oboInOwl:hasOBONamespace>
        <oboInOwl:id>GAZ:00043436</oboInOwl:id>
        <rdfs:label>Freak Island</rdfs:label>
    </owl:NamedIndividual>
    


    <!-- http://purl.obolibrary.org/obo/GAZ_00043437 -->

    <owl:NamedIndividual rdf:about="http://purl.obolibrary.org/obo/GAZ_00043437">
        <obo:RO_0001025 rdf:resource="http://purl.obolibrary.org/obo/GAZ_00017493"/>
        <oboInOwl:hasOBONamespace>GAZ</oboInOwl:hasOBONamespace>
        <oboInOwl:id>GAZ:00043437</oboInOwl:id>
        <rdfs:label>Bailey Island</rdfs:label>
    </owl:NamedIndividual>
    


    <!-- http://purl.obolibrary.org/obo/GAZ_00043438 -->

    <owl:NamedIndividual rdf:about="http://purl.obolibrary.org/obo/GAZ_00043438">
        <obo:RO_0001025 rdf:resource="http://purl.obolibrary.org/obo/GAZ_00017493"/>
        <oboInOwl:hasOBONamespace>GAZ</oboInOwl:hasOBONamespace>
        <oboInOwl:id>GAZ:00043438</oboInOwl:id>
        <rdfs:label>Sir Charles Metcalf Island</rdfs:label>
    </owl:NamedIndividual>
    


    <!-- http://purl.obolibrary.org/obo/GAZ_00043439 -->

    <owl:NamedIndividual rdf:about="http://purl.obolibrary.org/obo/GAZ_00043439">
        <obo:RO_0001025 rdf:resource="http://purl.obolibrary.org/obo/GAZ_00017493"/>
        <oboInOwl:hasOBONamespace>GAZ</oboInOwl:hasOBONamespace>
        <oboInOwl:id>GAZ:00043439</oboInOwl:id>
        <rdfs:label>Kabosa Island</rdfs:label>
    </owl:NamedIndividual>
    


    <!-- http://purl.obolibrary.org/obo/GAZ_00043440 -->

    <owl:NamedIndividual rdf:about="http://purl.obolibrary.org/obo/GAZ_00043440">
        <obo:RO_0001025 rdf:resource="http://purl.obolibrary.org/obo/GAZ_00017493"/>
        <oboInOwl:hasOBONamespace>GAZ</oboInOwl:hasOBONamespace>
        <oboInOwl:id>GAZ:00043440</oboInOwl:id>
        <rdfs:label>Blundell Island</rdfs:label>
    </owl:NamedIndividual>
    


    <!-- http://purl.obolibrary.org/obo/GAZ_00043441 -->

    <owl:NamedIndividual rdf:about="http://purl.obolibrary.org/obo/GAZ_00043441">
        <obo:RO_0001025 rdf:resource="http://purl.obolibrary.org/obo/GAZ_00017493"/>
        <obo:IAO_0000115>An island in the Mergui Archipelago, Burma.</obo:IAO_0000115>
        <oboInOwl:hasOBONamespace>GAZ</oboInOwl:hasOBONamespace>
        <oboInOwl:id>GAZ:00043441</oboInOwl:id>
        <rdfs:label>Thayawthadangyi Kyun</rdfs:label>
    </owl:NamedIndividual>
    


    <!-- http://purl.obolibrary.org/obo/GAZ_00043442 -->

    <owl:NamedIndividual rdf:about="http://purl.obolibrary.org/obo/GAZ_00043442">
        <obo:RO_0001025 rdf:resource="http://purl.obolibrary.org/obo/GAZ_00017493"/>
        <oboInOwl:hasOBONamespace>GAZ</oboInOwl:hasOBONamespace>
        <oboInOwl:id>GAZ:00043442</oboInOwl:id>
        <rdfs:label>Tenasserim Island</rdfs:label>
    </owl:NamedIndividual>
    


    <!-- http://purl.obolibrary.org/obo/GAZ_00043443 -->

    <owl:NamedIndividual rdf:about="http://purl.obolibrary.org/obo/GAZ_00043443">
        <obo:RO_0001025 rdf:resource="http://purl.obolibrary.org/obo/GAZ_00017493"/>
        <oboInOwl:hasOBONamespace>GAZ</oboInOwl:hasOBONamespace>
        <oboInOwl:id>GAZ:00043443</oboInOwl:id>
        <rdfs:label>West Canister Island</rdfs:label>
    </owl:NamedIndividual>
    


    <!-- http://purl.obolibrary.org/obo/GAZ_00045834 -->

    <owl:NamedIndividual rdf:about="http://purl.obolibrary.org/obo/GAZ_00045834">
        <obo:RO_0001025 rdf:resource="http://purl.obolibrary.org/obo/GAZ_00025550"/>
        <obo:IAO_0000115>An island off the coast of Myanmar.</obo:IAO_0000115>
        <oboInOwl:hasOBONamespace>GAZ</oboInOwl:hasOBONamespace>
        <oboInOwl:id>GAZ:00045834</oboInOwl:id>
        <rdfs:label>Ramree Island</rdfs:label>
    </owl:NamedIndividual>
    


    <!-- http://purl.obolibrary.org/obo/GAZ_00045843 -->

    <owl:NamedIndividual rdf:about="http://purl.obolibrary.org/obo/GAZ_00045843">
        <obo:RO_0001025 rdf:resource="http://purl.obolibrary.org/obo/GAZ_02000006"/>
        <obo:IAO_0000115>Islands located in the eastern Indian Ocean, politically administered by Myanmar under Yangon Division. Geographically, they are a part of the Andaman Islands archipelago and separated from the North Andaman Island (India) by the 20 km wide Coco channel. The Bay of Bengal lies to the west and the Andaman Sea to the east of the islands. The Burmese mainland is 300 km to the north.</obo:IAO_0000115>
        <oboInOwl:hasOBONamespace>GAZ</oboInOwl:hasOBONamespace>
        <oboInOwl:id>GAZ:00045843</oboInOwl:id>
        <rdfs:label>Coco Islands</rdfs:label>
    </owl:NamedIndividual>
    


    <!-- http://purl.obolibrary.org/obo/GAZ_00046069 -->

    <owl:NamedIndividual rdf:about="http://purl.obolibrary.org/obo/GAZ_00046069">
        <obo:RO_0001025 rdf:resource="http://purl.obolibrary.org/obo/GAZ_00045843"/>
        <obo:IAO_0000115>One of the Coco Islands. It lies 15 km to the southwest from the Great Coco Island.</obo:IAO_0000115>
        <oboInOwl:hasOBONamespace>GAZ</oboInOwl:hasOBONamespace>
        <oboInOwl:id>GAZ:00046069</oboInOwl:id>
        <rdfs:label>Little Coco Island</rdfs:label>
    </owl:NamedIndividual>
    


    <!-- http://purl.obolibrary.org/obo/GAZ_00046070 -->

    <owl:NamedIndividual rdf:about="http://purl.obolibrary.org/obo/GAZ_00046070">
        <obo:RO_0001025 rdf:resource="http://purl.obolibrary.org/obo/GAZ_00045843"/>
        <obo:IAO_0000115>One of the Coco Islands.</obo:IAO_0000115>
        <oboInOwl:hasOBONamespace>GAZ</oboInOwl:hasOBONamespace>
        <oboInOwl:id>GAZ:00046070</oboInOwl:id>
        <rdfs:label>Great Coco Island</rdfs:label>
    </owl:NamedIndividual>
    


    <!-- http://purl.obolibrary.org/obo/GAZ_00046071 -->

    <owl:NamedIndividual rdf:about="http://purl.obolibrary.org/obo/GAZ_00046071">
        <obo:RO_0001025 rdf:resource="http://purl.obolibrary.org/obo/GAZ_00025550"/>
        <obo:IAO_0000115>An island in the Bay of Bengal close to Ramree Island belonging to Burma. Situated in the Rakhine State it has an area of approximately 500 km2.</obo:IAO_0000115>
        <oboInOwl:hasOBONamespace>GAZ</oboInOwl:hasOBONamespace>
        <oboInOwl:id>GAZ:00046071</oboInOwl:id>
        <rdfs:label>Cheduba Island</rdfs:label>
    </owl:NamedIndividual>
    


    <!-- http://purl.obolibrary.org/obo/GAZ_00048759 -->

    <owl:NamedIndividual rdf:about="http://purl.obolibrary.org/obo/GAZ_00048759">
        <obo:RO_0001025 rdf:resource="http://purl.obolibrary.org/obo/GAZ_00017493"/>
        <obo:IAO_0000115>An island in the Mergui Archipelago, Burma (Myanmar).</obo:IAO_0000115>
        <oboInOwl:hasOBONamespace>GAZ</oboInOwl:hasOBONamespace>
        <oboInOwl:id>GAZ:00048759</oboInOwl:id>
        <rdfs:label>Kadetkyi Kyun</rdfs:label>
    </owl:NamedIndividual>
    


    <!-- http://purl.obolibrary.org/obo/GAZ_00048760 -->

    <owl:NamedIndividual rdf:about="http://purl.obolibrary.org/obo/GAZ_00048760">
        <obo:RO_0001025 rdf:resource="http://purl.obolibrary.org/obo/GAZ_00017493"/>
        <obo:IAO_0000115>An island in the Mergui Archipelago, Burma.</obo:IAO_0000115>
        <oboInOwl:hasOBONamespace>GAZ</oboInOwl:hasOBONamespace>
        <oboInOwl:id>GAZ:00048760</oboInOwl:id>
        <rdfs:label>Lanbi Kyun</rdfs:label>
    </owl:NamedIndividual>
    


    <!-- http://purl.obolibrary.org/obo/GAZ_00048761 -->

    <owl:NamedIndividual rdf:about="http://purl.obolibrary.org/obo/GAZ_00048761">
        <obo:RO_0001025 rdf:resource="http://purl.obolibrary.org/obo/GAZ_00006899"/>
        <oboInOwl:hasOBONamespace>GAZ</oboInOwl:hasOBONamespace>
        <oboInOwl:id>GAZ:00048761</oboInOwl:id>
        <rdfs:label>Bilugyun Island</rdfs:label>
    </owl:NamedIndividual>
    


    <!-- http://purl.obolibrary.org/obo/GAZ_00048762 -->

    <owl:NamedIndividual rdf:about="http://purl.obolibrary.org/obo/GAZ_00048762">
        <obo:RO_0001025 rdf:resource="http://purl.obolibrary.org/obo/GAZ_00006899"/>
        <obo:IAO_0000115>An island N of the Great Coco Island and S of the Irrawaddy Delta.</obo:IAO_0000115>
        <oboInOwl:hasOBONamespace>GAZ</oboInOwl:hasOBONamespace>
        <oboInOwl:id>GAZ:00048762</oboInOwl:id>
        <rdfs:label>Preparis Island</rdfs:label>
    </owl:NamedIndividual>
    


    <!-- http://purl.obolibrary.org/obo/GAZ_00048763 -->

    <owl:NamedIndividual rdf:about="http://purl.obolibrary.org/obo/GAZ_00048763">
        <obo:RO_0001025 rdf:resource="http://purl.obolibrary.org/obo/GAZ_00045843"/>
        <obo:IAO_0000115>One of the Coco Islands.</obo:IAO_0000115>
        <oboInOwl:hasOBONamespace>GAZ</oboInOwl:hasOBONamespace>
        <oboInOwl:id>GAZ:00048763</oboInOwl:id>
        <rdfs:label>Table Island</rdfs:label>
    </owl:NamedIndividual>
    


    <!-- http://purl.obolibrary.org/obo/GAZ_00049340 -->

    <owl:NamedIndividual rdf:about="http://purl.obolibrary.org/obo/GAZ_00049340">
        <oboInOwl:hasOBONamespace>GAZ</oboInOwl:hasOBONamespace>
        <oboInOwl:id>GAZ:00049340</oboInOwl:id>
        <rdfs:label>Khong Island</rdfs:label>
    </owl:NamedIndividual>
    


    <!-- http://purl.obolibrary.org/obo/GAZ_00054351 -->

    <owl:NamedIndividual rdf:about="http://purl.obolibrary.org/obo/GAZ_00054351">
        <obo:RO_0001025 rdf:resource="http://purl.obolibrary.org/obo/GAZ_00247734"/>
        <obo:IAO_0000115>A large, steep-sided composite stratovolcanic cone that rises 1150 m above a surrounding lava plateau to a height of 1518 m. The main edifice consists of overlapping basaltic and basaltic-andesite lava flows, pyroclastic deposits, and scoriaceous material originating from strombolian eruptions that may have dominated later stages of the volcano&apos;s growth. Mount Popa contains a 1.6 km wide, 850-m-deep horseshoe-shaped caldera that is widely breached to the NW and formed as a result of slope failure. A 3 cu km debris-avalanche deposit covers an area of 27 km2 north of the breach.</obo:IAO_0000115>
        <oboInOwl:hasOBONamespace>GAZ</oboInOwl:hasOBONamespace>
        <oboInOwl:id>GAZ:00054351</oboInOwl:id>
        <rdfs:label>Mount Popa</rdfs:label>
    </owl:NamedIndividual>
    


    <!-- http://purl.obolibrary.org/obo/GAZ_00054352 -->

    <owl:NamedIndividual rdf:about="http://purl.obolibrary.org/obo/GAZ_00054352">
        <obo:RO_0001025 rdf:resource="http://purl.obolibrary.org/obo/GAZ_00006899"/>
        <obo:IAO_0000115>A volcanic field that contains seven or eight late-Pliocene and Pleistocene explosion craters. Scattered outcrops of basaltic lava flows are found in this area, including an undated, but very recent basalt that forms a plateau north of Thayet-Pingan. A lake-filled crater located at Songyuang is surrounded by olivine basaltic lava flows and pyroclastic material. This region along the lower Chindwin River also contains rhyolitic, dacitic, and andesitic rocks.</obo:IAO_0000115>
        <oboInOwl:hasOBONamespace>GAZ</oboInOwl:hasOBONamespace>
        <oboInOwl:id>GAZ:00054352</oboInOwl:id>
        <rdfs:label>Lower Chindwin Volcanic Field</rdfs:label>
    </owl:NamedIndividual>
    


    <!-- http://purl.obolibrary.org/obo/GAZ_00054353 -->

    <owl:NamedIndividual rdf:about="http://purl.obolibrary.org/obo/GAZ_00054353">
        <obo:RO_0001025 rdf:resource="http://purl.obolibrary.org/obo/GAZ_00006899"/>
        <obo:IAO_0000115>A volcanic plateau located in central Burma, south of Mandalay, covering an area of 62 km2. The lava flows originated from fissure vents.</obo:IAO_0000115>
        <oboInOwl:hasOBONamespace>GAZ</oboInOwl:hasOBONamespace>
        <oboInOwl:id>GAZ:00054353</oboInOwl:id>
        <rdfs:label>Singu Plateau</rdfs:label>
    </owl:NamedIndividual>
    


    <!-- http://purl.obolibrary.org/obo/GAZ_00056889 -->

    <owl:NamedIndividual rdf:about="http://purl.obolibrary.org/obo/GAZ_00056889">
        <rdf:type rdf:resource="http://purl.obolibrary.org/obo/ENVO_00000106"/>
        <obo:IAO_0000115>A range of hills in northwestern Myanmar that extend into India&apos;s Manipur state.</obo:IAO_0000115>
        <oboInOwl:hasOBONamespace>GAZ</oboInOwl:hasOBONamespace>
        <oboInOwl:id>GAZ:00056889</oboInOwl:id>
        <rdfs:label>Chin Hills</rdfs:label>
    </owl:NamedIndividual>
    


    <!-- http://purl.obolibrary.org/obo/GAZ_00056890 -->

    <owl:NamedIndividual rdf:about="http://purl.obolibrary.org/obo/GAZ_00056890">
        <obo:IAO_0000115>The hills on India&apos;s eastern border with Myanmar.</obo:IAO_0000115>
        <oboInOwl:hasOBONamespace>GAZ</oboInOwl:hasOBONamespace>
        <oboInOwl:id>GAZ:00056890</oboInOwl:id>
        <rdfs:label>Patkai Hills</rdfs:label>
    </owl:NamedIndividual>
    


    <!-- http://purl.obolibrary.org/obo/GAZ_00056892 -->

    <owl:NamedIndividual rdf:about="http://purl.obolibrary.org/obo/GAZ_00056892">
        <obo:RO_0001025 rdf:resource="http://purl.obolibrary.org/obo/GAZ_00056890"/>
        <obo:IAO_0000115>Part of the Patkai range.</obo:IAO_0000115>
        <oboInOwl:hasOBONamespace>GAZ</oboInOwl:hasOBONamespace>
        <oboInOwl:id>GAZ:00056892</oboInOwl:id>
        <rdfs:label>Garo-Khasi-Jaintia Hills</rdfs:label>
    </owl:NamedIndividual>
    


    <!-- http://purl.obolibrary.org/obo/GAZ_00056893 -->

    <owl:NamedIndividual rdf:about="http://purl.obolibrary.org/obo/GAZ_00056893">
        <obo:RO_0001025 rdf:resource="http://purl.obolibrary.org/obo/GAZ_00056890"/>
        <obo:IAO_0000115>Part of the Patkai range.</obo:IAO_0000115>
        <oboInOwl:hasOBONamespace>GAZ</oboInOwl:hasOBONamespace>
        <oboInOwl:id>GAZ:00056893</oboInOwl:id>
        <rdfs:label>Patkai-Bum Hills</rdfs:label>
    </owl:NamedIndividual>
    


    <!-- http://purl.obolibrary.org/obo/GAZ_00057337 -->

    <owl:NamedIndividual rdf:about="http://purl.obolibrary.org/obo/GAZ_00057337">
        <obo:RO_0001025 rdf:resource="http://purl.obolibrary.org/obo/GAZ_00006899"/>
        <obo:IAO_0000115>A mountain range in Southeast Asia (Latitude: 27deg30minN, Longitude: 99deg0minE) that forms the border between Burma and Yunnan, China. The Hengduan Shan chain of mountains runs roughly north to south, defining the eastern edge of the Tibetan Plateau.</obo:IAO_0000115>
        <oboInOwl:hasOBONamespace>GAZ</oboInOwl:hasOBONamespace>
        <oboInOwl:id>GAZ:00057337</oboInOwl:id>
        <rdfs:label>Hengduan Shan Range</rdfs:label>
    </owl:NamedIndividual>
    


    <!-- http://purl.obolibrary.org/obo/GAZ_00058186 -->

    <owl:NamedIndividual rdf:about="http://purl.obolibrary.org/obo/GAZ_00058186">
        <obo:RO_0001025 rdf:resource="http://purl.obolibrary.org/obo/GAZ_00058187"/>
        <obo:RO_0001025 rdf:resource="http://purl.obolibrary.org/obo/GAZ_00058188"/>
        <obo:IAO_0000115>A freshwater lake located in Mohnyin Township in the Kachin State of Burma.</obo:IAO_0000115>
        <oboInOwl:hasOBONamespace>GAZ</oboInOwl:hasOBONamespace>
        <oboInOwl:id>GAZ:00058186</oboInOwl:id>
        <rdfs:label>Indawgyi Lake</rdfs:label>
    </owl:NamedIndividual>
    


    <!-- http://purl.obolibrary.org/obo/GAZ_00058187 -->

    <owl:NamedIndividual rdf:about="http://purl.obolibrary.org/obo/GAZ_00058187">
        <obo:RO_0001025 rdf:resource="http://purl.obolibrary.org/obo/GAZ_02000012"/>
        <obo:IAO_0000115>A protected area.</obo:IAO_0000115>
        <oboInOwl:hasOBONamespace>GAZ</oboInOwl:hasOBONamespace>
        <oboInOwl:id>GAZ:00058187</oboInOwl:id>
        <rdfs:label>Indawgyi Lake Wildlife Sanctuary</rdfs:label>
    </owl:NamedIndividual>
    


    <!-- http://purl.obolibrary.org/obo/GAZ_00058188 -->

    <owl:NamedIndividual rdf:about="http://purl.obolibrary.org/obo/GAZ_00058188">
        <obo:RO_0001025 rdf:resource="http://purl.obolibrary.org/obo/GAZ_02000012"/>
        <oboInOwl:hasOBONamespace>GAZ</oboInOwl:hasOBONamespace>
        <oboInOwl:id>GAZ:00058188</oboInOwl:id>
        <rdfs:label>Mohnyin Township</rdfs:label>
    </owl:NamedIndividual>
    


    <!-- http://purl.obolibrary.org/obo/GAZ_00058189 -->

    <owl:NamedIndividual rdf:about="http://purl.obolibrary.org/obo/GAZ_00058189">
        <obo:RO_0001025 rdf:resource="http://purl.obolibrary.org/obo/GAZ_00118425"/>
        <obo:IAO_0000115>A freshwater lake located in the mountains of Shan State in Myanmar. The watershed area for the lake lies to a large extent to the north and west of the lake. The lake drains through the Nam Pilu or Balu Chaung on its southern end. There is a hot spring on its northwestern shore.</obo:IAO_0000115>
        <oboInOwl:hasOBONamespace>GAZ</oboInOwl:hasOBONamespace>
        <oboInOwl:id>GAZ:00058189</oboInOwl:id>
        <rdfs:label>Inle Lake</rdfs:label>
    </owl:NamedIndividual>
    


    <!-- http://purl.obolibrary.org/obo/GAZ_00058190 -->

    <owl:NamedIndividual rdf:about="http://purl.obolibrary.org/obo/GAZ_00058190">
        <obo:RO_0001025 rdf:resource="http://purl.obolibrary.org/obo/GAZ_00118644"/>
        <obo:IAO_0000115>A lake in Yangon. It is an artificial lake expanded as a water reservoir in about 1882 to 1883. Water from Inya Lake is channelled through a series of pipes to Kandawgyi Lake.</obo:IAO_0000115>
        <oboInOwl:hasOBONamespace>GAZ</oboInOwl:hasOBONamespace>
        <oboInOwl:id>GAZ:00058190</oboInOwl:id>
        <rdfs:label>Inya Lake</rdfs:label>
    </owl:NamedIndividual>
    


    <!-- http://purl.obolibrary.org/obo/GAZ_00058191 -->

    <owl:NamedIndividual rdf:about="http://purl.obolibrary.org/obo/GAZ_00058191">
        <obo:RO_0001025 rdf:resource="http://purl.obolibrary.org/obo/GAZ_02000006"/>
        <obo:IAO_0000115>An artificial lake in Yangon. Water from Inya Lake is channelled through a series of pipes to Kandawgyi Lake.</obo:IAO_0000115>
        <oboInOwl:hasOBONamespace>GAZ</oboInOwl:hasOBONamespace>
        <oboInOwl:id>GAZ:00058191</oboInOwl:id>
        <rdfs:label>Kandawgyi Lake</rdfs:label>
    </owl:NamedIndividual>
    


    <!-- http://purl.obolibrary.org/obo/GAZ_00058192 -->

    <owl:NamedIndividual rdf:about="http://purl.obolibrary.org/obo/GAZ_00058192">
        <obo:RO_0001025 rdf:resource="http://purl.obolibrary.org/obo/GAZ_00006899"/>
        <obo:IAO_0000115>A small body of water lying south of Pangsau village, the first habitation in Burma (Myanmar) on the Ledo Road, 2 km east of the Pangsau Pass on the India-Burma border.</obo:IAO_0000115>
        <oboInOwl:hasOBONamespace>GAZ</oboInOwl:hasOBONamespace>
        <oboInOwl:id>GAZ:00058192</oboInOwl:id>
        <rdfs:label>Lake of No Return</rdfs:label>
    </owl:NamedIndividual>
    


    <!-- http://purl.obolibrary.org/obo/GAZ_00115117 -->

    <owl:NamedIndividual rdf:about="http://purl.obolibrary.org/obo/GAZ_00115117">
        <obo:RO_0001025 rdf:resource="http://purl.obolibrary.org/obo/GAZ_00118408"/>
        <obo:RO_0001025 rdf:resource="http://purl.obolibrary.org/obo/GAZ_02000002"/>
        <obo:IAO_0000115>The lowest expanse of land in Burma that fans out from the limit of tidal influence at Myan Aung to the Bay of Bengal and Andaman Sea, 290 km to the south at the mouth of the Ayeyarwady River. The Irrawaddy Delta comprises the main arms of Pathein River, Pyapon River, Bogale River, and Toe River. It is bounded to the west by the southern Arakan Yoma range and to the east by the Pegu Yoma. The city of Rangoon, situated on the southermost spur of the Pegu Yoma, lies at the southeastern edge of the delta.</obo:IAO_0000115>
        <oboInOwl:hasOBONamespace>GAZ</oboInOwl:hasOBONamespace>
        <oboInOwl:id>GAZ:00115117</oboInOwl:id>
        <rdfs:label>Irrawaddy Delta</rdfs:label>
    </owl:NamedIndividual>
    


    <!-- http://purl.obolibrary.org/obo/GAZ_00118408 -->

    <owl:NamedIndividual rdf:about="http://purl.obolibrary.org/obo/GAZ_00118408">
        <obo:RO_0001025 rdf:resource="http://purl.obolibrary.org/obo/GAZ_00006899"/>
        <obo:IAO_0000115>A river that flows from North to South of Burma (Myanmar). The Ayeyarwaddy River starts in the North of Kachin State, at the confluence of the Mali Hka and N&apos;Mai Hka rivers. The western Mali Hka branch arises from the end of the southern Himalayas, north of Putao. The Ayeyarwaddy River bisects the country from north to south and empties through a nine-armed Irrawaddy Delta into the Indian Ocean.</obo:IAO_0000115>
        <oboInOwl:hasOBONamespace>GAZ</oboInOwl:hasOBONamespace>
        <oboInOwl:id>GAZ:00118408</oboInOwl:id>
        <rdfs:label>Irrawaddy River</rdfs:label>
    </owl:NamedIndividual>
    


    <!-- http://purl.obolibrary.org/obo/GAZ_00118409 -->

    <owl:NamedIndividual rdf:about="http://purl.obolibrary.org/obo/GAZ_00118409">
        <obo:RO_0001025 rdf:resource="http://purl.obolibrary.org/obo/GAZ_00115117"/>
        <obo:IAO_0000115>An island in the Irrawaddy Delta.</obo:IAO_0000115>
        <oboInOwl:hasOBONamespace>GAZ</oboInOwl:hasOBONamespace>
        <oboInOwl:id>GAZ:00118409</oboInOwl:id>
        <rdfs:label>Haigyi Kyun</rdfs:label>
    </owl:NamedIndividual>
    


    <!-- http://purl.obolibrary.org/obo/GAZ_00118410 -->

    <owl:NamedIndividual rdf:about="http://purl.obolibrary.org/obo/GAZ_00118410">
        <obo:RO_0001025 rdf:resource="http://purl.obolibrary.org/obo/GAZ_00115117"/>
        <obo:IAO_0000115>An island in the Irrawaddy Delta.</obo:IAO_0000115>
        <oboInOwl:hasOBONamespace>GAZ</oboInOwl:hasOBONamespace>
        <oboInOwl:id>GAZ:00118410</oboInOwl:id>
        <rdfs:label>Leit Kyun</rdfs:label>
    </owl:NamedIndividual>
    


    <!-- http://purl.obolibrary.org/obo/GAZ_00118412 -->

    <owl:NamedIndividual rdf:about="http://purl.obolibrary.org/obo/GAZ_00118412">
        <obo:RO_0001025 rdf:resource="http://purl.obolibrary.org/obo/GAZ_00115117"/>
        <obo:IAO_0000115>An island in the Irrawaddy Delta.</obo:IAO_0000115>
        <oboInOwl:hasOBONamespace>GAZ</oboInOwl:hasOBONamespace>
        <oboInOwl:id>GAZ:00118412</oboInOwl:id>
        <rdfs:label>Pyin Salu Kyun</rdfs:label>
    </owl:NamedIndividual>
    


    <!-- http://purl.obolibrary.org/obo/GAZ_00118414 -->

    <owl:NamedIndividual rdf:about="http://purl.obolibrary.org/obo/GAZ_00118414">
        <obo:RO_0001025 rdf:resource="http://purl.obolibrary.org/obo/GAZ_02000012"/>
        <obo:IAO_0000115>A mountain range in the northeastern province of Kachin State in Burma.</obo:IAO_0000115>
        <oboInOwl:hasOBONamespace>GAZ</oboInOwl:hasOBONamespace>
        <oboInOwl:id>GAZ:00118414</oboInOwl:id>
        <rdfs:label>Kumon Bum Mountains</rdfs:label>
    </owl:NamedIndividual>
    


    <!-- http://purl.obolibrary.org/obo/GAZ_00118415 -->

    <owl:NamedIndividual rdf:about="http://purl.obolibrary.org/obo/GAZ_00118415">
        <obo:RO_0001025 rdf:resource="http://purl.obolibrary.org/obo/GAZ_02000012"/>
        <obo:IAO_0000115>A protected area. Established 1998-11-10.</obo:IAO_0000115>
        <oboInOwl:hasOBONamespace>GAZ</oboInOwl:hasOBONamespace>
        <oboInOwl:id>GAZ:00118415</oboInOwl:id>
        <rdfs:label>Hkakabo Razi National Park</rdfs:label>
    </owl:NamedIndividual>
    


    <!-- http://purl.obolibrary.org/obo/GAZ_00118416 -->

    <owl:NamedIndividual rdf:about="http://purl.obolibrary.org/obo/GAZ_00118416">
        <obo:RO_0001025 rdf:resource="http://purl.obolibrary.org/obo/GAZ_02000007"/>
        <obo:IAO_0000115>A plateau in eastern Myanmar.</obo:IAO_0000115>
        <oboInOwl:hasOBONamespace>GAZ</oboInOwl:hasOBONamespace>
        <oboInOwl:id>GAZ:00118416</oboInOwl:id>
        <rdfs:label>Shan Plateau</rdfs:label>
    </owl:NamedIndividual>
    


    <!-- http://purl.obolibrary.org/obo/GAZ_00118417 -->

    <owl:NamedIndividual rdf:about="http://purl.obolibrary.org/obo/GAZ_00118417">
        <obo:RO_0001025 rdf:resource="http://purl.obolibrary.org/obo/GAZ_02000012"/>
        <obo:IAO_0000115>A heavily forested group of highlands in the extreme northeastern of the Kachin State of Burma.</obo:IAO_0000115>
        <oboInOwl:hasOBONamespace>GAZ</oboInOwl:hasOBONamespace>
        <oboInOwl:id>GAZ:00118417</oboInOwl:id>
        <rdfs:label>Kachin Hills</rdfs:label>
    </owl:NamedIndividual>
    


    <!-- http://purl.obolibrary.org/obo/GAZ_00118418 -->

    <owl:NamedIndividual rdf:about="http://purl.obolibrary.org/obo/GAZ_00118418">
        <obo:RO_0001025 rdf:resource="http://purl.obolibrary.org/obo/GAZ_02000003"/>
        <obo:IAO_0000115>The largest national park in Myanmar (also known as Burma). The park consists of the Patolon Reserved Forest and the adijoining Taungdwin Reserved Forest. The area of the National Park comprise the upper catchment basins of the Patolon and Taungdwin rivers, both of which are northward valleys separated from each other and from adjoining valleys to the west and east by long North-South ridges at an elevation of about 2000 to over 4000 ft. Established 1984.</obo:IAO_0000115>
        <oboInOwl:hasOBONamespace>GAZ</oboInOwl:hasOBONamespace>
        <oboInOwl:id>GAZ:00118418</oboInOwl:id>
        <rdfs:label>Alaungdaw Kathapa National Park</rdfs:label>
    </owl:NamedIndividual>
    


    <!-- http://purl.obolibrary.org/obo/GAZ_00118419 -->

    <owl:NamedIndividual rdf:about="http://purl.obolibrary.org/obo/GAZ_00118419">
        <obo:RO_0001025 rdf:resource="http://purl.obolibrary.org/obo/GAZ_02000012"/>
        <obo:IAO_0000115>A national park.</obo:IAO_0000115>
        <oboInOwl:hasOBONamespace>GAZ</oboInOwl:hasOBONamespace>
        <oboInOwl:id>GAZ:00118419</oboInOwl:id>
        <rdfs:label>Khakaborazi National Park</rdfs:label>
    </owl:NamedIndividual>
    


    <!-- http://purl.obolibrary.org/obo/GAZ_00118420 -->

    <owl:NamedIndividual rdf:about="http://purl.obolibrary.org/obo/GAZ_00118420">
        <obo:RO_0001025 rdf:resource="http://purl.obolibrary.org/obo/GAZ_02000003"/>
        <obo:IAO_0000115>A protected area.</obo:IAO_0000115>
        <oboInOwl:hasOBONamespace>GAZ</oboInOwl:hasOBONamespace>
        <oboInOwl:id>GAZ:00118420</oboInOwl:id>
        <rdfs:label>Chatthin Wildlife Sanctuary</rdfs:label>
    </owl:NamedIndividual>
    


    <!-- http://purl.obolibrary.org/obo/GAZ_00118421 -->

    <owl:NamedIndividual rdf:about="http://purl.obolibrary.org/obo/GAZ_00118421">
        <obo:RO_0001025 rdf:resource="http://purl.obolibrary.org/obo/GAZ_02000003"/>
        <obo:IAO_0000115>A protected area.</obo:IAO_0000115>
        <oboInOwl:hasOBONamespace>GAZ</oboInOwl:hasOBONamespace>
        <oboInOwl:id>GAZ:00118421</oboInOwl:id>
        <rdfs:label>Hukawng Valley Tiger Reserve</rdfs:label>
    </owl:NamedIndividual>
    


    <!-- http://purl.obolibrary.org/obo/GAZ_00118422 -->

    <owl:NamedIndividual rdf:about="http://purl.obolibrary.org/obo/GAZ_00118422">
        <obo:RO_0001025 rdf:resource="http://purl.obolibrary.org/obo/GAZ_02000010"/>
        <obo:IAO_0000115>A protected area.</obo:IAO_0000115>
        <oboInOwl:hasOBONamespace>GAZ</oboInOwl:hasOBONamespace>
        <oboInOwl:id>GAZ:00118422</oboInOwl:id>
        <rdfs:label>Rakhine Yoma Elephant Reserve</rdfs:label>
    </owl:NamedIndividual>
    


    <!-- http://purl.obolibrary.org/obo/GAZ_00118423 -->

    <owl:NamedIndividual rdf:about="http://purl.obolibrary.org/obo/GAZ_00118423">
        <obo:RO_0001025 rdf:resource="http://purl.obolibrary.org/obo/GAZ_02000013"/>
        <obo:IAO_0000115>A national park.</obo:IAO_0000115>
        <oboInOwl:hasOBONamespace>GAZ</oboInOwl:hasOBONamespace>
        <oboInOwl:id>GAZ:00118423</oboInOwl:id>
        <rdfs:label>Mount Victoria National Park</rdfs:label>
    </owl:NamedIndividual>
    


    <!-- http://purl.obolibrary.org/obo/GAZ_00118424 -->

    <owl:NamedIndividual rdf:about="http://purl.obolibrary.org/obo/GAZ_00118424">
        <obo:RO_0001025 rdf:resource="http://purl.obolibrary.org/obo/GAZ_02000001"/>
        <obo:IAO_0000115>A national park.</obo:IAO_0000115>
        <oboInOwl:hasOBONamespace>GAZ</oboInOwl:hasOBONamespace>
        <oboInOwl:id>GAZ:00118424</oboInOwl:id>
        <rdfs:label>Popa Mountain National Park</rdfs:label>
    </owl:NamedIndividual>
    


    <!-- http://purl.obolibrary.org/obo/GAZ_00118425 -->

    <owl:NamedIndividual rdf:about="http://purl.obolibrary.org/obo/GAZ_00118425">
        <obo:RO_0001025 rdf:resource="http://purl.obolibrary.org/obo/GAZ_00247041"/>
        <obo:IAO_0000115>A protected area.</obo:IAO_0000115>
        <oboInOwl:hasOBONamespace>GAZ</oboInOwl:hasOBONamespace>
        <oboInOwl:id>GAZ:00118425</oboInOwl:id>
        <rdfs:label>Inlay Lake Wetland Sanctuary</rdfs:label>
    </owl:NamedIndividual>
    


    <!-- http://purl.obolibrary.org/obo/GAZ_00118426 -->

    <owl:NamedIndividual rdf:about="http://purl.obolibrary.org/obo/GAZ_00118426">
        <obo:RO_0001025 rdf:resource="http://purl.obolibrary.org/obo/GAZ_02000005"/>
        <obo:IAO_0000115>A protected area.</obo:IAO_0000115>
        <oboInOwl:hasOBONamespace>GAZ</oboInOwl:hasOBONamespace>
        <oboInOwl:id>GAZ:00118426</oboInOwl:id>
        <rdfs:label>Shwesettaw Wildlife Reserve</rdfs:label>
    </owl:NamedIndividual>
    


    <!-- http://purl.obolibrary.org/obo/GAZ_00118427 -->

    <owl:NamedIndividual rdf:about="http://purl.obolibrary.org/obo/GAZ_00118427">
        <obo:RO_0001025 rdf:resource="http://purl.obolibrary.org/obo/GAZ_02000004"/>
        <obo:IAO_0000115>A protected area.</obo:IAO_0000115>
        <oboInOwl:hasOBONamespace>GAZ</oboInOwl:hasOBONamespace>
        <oboInOwl:id>GAZ:00118427</oboInOwl:id>
        <rdfs:label>Sein Ye Forest Park</rdfs:label>
    </owl:NamedIndividual>
    


    <!-- http://purl.obolibrary.org/obo/GAZ_00118428 -->

    <owl:NamedIndividual rdf:about="http://purl.obolibrary.org/obo/GAZ_00118428">
        <obo:RO_0001025 rdf:resource="http://purl.obolibrary.org/obo/GAZ_02000004"/>
        <obo:IAO_0000115>A protected area.</obo:IAO_0000115>
        <oboInOwl:hasOBONamespace>GAZ</oboInOwl:hasOBONamespace>
        <oboInOwl:id>GAZ:00118428</oboInOwl:id>
        <rdfs:label>Moneyingyi Wetland Sactuary</rdfs:label>
    </owl:NamedIndividual>
    


    <!-- http://purl.obolibrary.org/obo/GAZ_00118429 -->

    <owl:NamedIndividual rdf:about="http://purl.obolibrary.org/obo/GAZ_00118429">
        <obo:RO_0001025 rdf:resource="http://purl.obolibrary.org/obo/GAZ_02000006"/>
        <obo:IAO_0000115>A protected area.</obo:IAO_0000115>
        <oboInOwl:hasOBONamespace>GAZ</oboInOwl:hasOBONamespace>
        <oboInOwl:id>GAZ:00118429</oboInOwl:id>
        <rdfs:label>Myaing Hay Wun Elephant Park</rdfs:label>
    </owl:NamedIndividual>
    


    <!-- http://purl.obolibrary.org/obo/GAZ_00118430 -->

    <owl:NamedIndividual rdf:about="http://purl.obolibrary.org/obo/GAZ_00118430">
        <obo:RO_0001025 rdf:resource="http://purl.obolibrary.org/obo/GAZ_02000000"/>
        <obo:IAO_0000115>A protected area.</obo:IAO_0000115>
        <oboInOwl:hasOBONamespace>GAZ</oboInOwl:hasOBONamespace>
        <oboInOwl:id>GAZ:00118430</oboInOwl:id>
        <rdfs:label>Lampi Kyun Wildlife Reserve</rdfs:label>
    </owl:NamedIndividual>
    


    <!-- http://purl.obolibrary.org/obo/GAZ_00118431 -->

    <owl:NamedIndividual rdf:about="http://purl.obolibrary.org/obo/GAZ_00118431">
        <obo:RO_0001025 rdf:resource="http://purl.obolibrary.org/obo/GAZ_00025539"/>
        <obo:IAO_0000115>A protected area. Located approximately 20 km west of Myitkyina, on the west bank of the Irrawaddy River in Myitkyina Forest Division, Kachin State.</obo:IAO_0000115>
        <oboInOwl:hasOBONamespace>GAZ</oboInOwl:hasOBONamespace>
        <oboInOwl:id>GAZ:00118431</oboInOwl:id>
        <rdfs:label>Pitaung Wildlife Reserve</rdfs:label>
    </owl:NamedIndividual>
    


    <!-- http://purl.obolibrary.org/obo/GAZ_00118432 -->

    <owl:NamedIndividual rdf:about="http://purl.obolibrary.org/obo/GAZ_00118432">
        <obo:RO_0001025 rdf:resource="http://purl.obolibrary.org/obo/GAZ_02000007"/>
        <obo:IAO_0000115>A national park.</obo:IAO_0000115>
        <oboInOwl:hasOBONamespace>GAZ</oboInOwl:hasOBONamespace>
        <oboInOwl:id>GAZ:00118432</oboInOwl:id>
        <rdfs:label>Loimwe National Park</rdfs:label>
    </owl:NamedIndividual>
    


    <!-- http://purl.obolibrary.org/obo/GAZ_00118433 -->

    <owl:NamedIndividual rdf:about="http://purl.obolibrary.org/obo/GAZ_00118433">
        <obo:RO_0001025 rdf:resource="http://purl.obolibrary.org/obo/GAZ_02000007"/>
        <obo:IAO_0000115>A protected area.</obo:IAO_0000115>
        <oboInOwl:hasOBONamespace>GAZ</oboInOwl:hasOBONamespace>
        <oboInOwl:id>GAZ:00118433</oboInOwl:id>
        <rdfs:label>Pasa Wildlife Reserve</rdfs:label>
    </owl:NamedIndividual>
    


    <!-- http://purl.obolibrary.org/obo/GAZ_00118434 -->

    <owl:NamedIndividual rdf:about="http://purl.obolibrary.org/obo/GAZ_00118434">
        <obo:RO_0001025 rdf:resource="http://purl.obolibrary.org/obo/GAZ_02000003"/>
        <obo:IAO_0000115>A protected area.</obo:IAO_0000115>
        <oboInOwl:hasOBONamespace>GAZ</oboInOwl:hasOBONamespace>
        <oboInOwl:id>GAZ:00118434</oboInOwl:id>
        <rdfs:label>Tamanthi Wildlife Reserve</rdfs:label>
    </owl:NamedIndividual>
    


    <!-- http://purl.obolibrary.org/obo/GAZ_00118435 -->

    <owl:NamedIndividual rdf:about="http://purl.obolibrary.org/obo/GAZ_00118435">
        <rdf:type rdf:resource="http://purl.obolibrary.org/obo/ENVO_00000004"/>
        <obo:RO_0001025 rdf:resource="http://purl.obolibrary.org/obo/GAZ_02000013"/>
        <obo:IAO_0000115>A district in Chin State, northwestern part of Myanmar. Tedim was previously in Falam District.</obo:IAO_0000115>
        <oboInOwl:hasOBONamespace>GAZ</oboInOwl:hasOBONamespace>
        <oboInOwl:id>GAZ:00118435</oboInOwl:id>
        <rdfs:label>Tedim District</rdfs:label>
    </owl:NamedIndividual>
    


    <!-- http://purl.obolibrary.org/obo/GAZ_00118436 -->

    <owl:NamedIndividual rdf:about="http://purl.obolibrary.org/obo/GAZ_00118436">
        <obo:RO_0001025 rdf:resource="http://purl.obolibrary.org/obo/GAZ_00118435"/>
        <oboInOwl:hasOBONamespace>GAZ</oboInOwl:hasOBONamespace>
        <oboInOwl:id>GAZ:00118436</oboInOwl:id>
        <rdfs:label>Tedim Township</rdfs:label>
    </owl:NamedIndividual>
    


    <!-- http://purl.obolibrary.org/obo/GAZ_00118437 -->

    <owl:NamedIndividual rdf:about="http://purl.obolibrary.org/obo/GAZ_00118437">
        <obo:RO_0001025 rdf:resource="http://purl.obolibrary.org/obo/GAZ_00025538"/>
        <obo:IAO_0000115>A populated place. A township of Falam District in the Chin State of Myanmar.</obo:IAO_0000115>
        <oboInOwl:hasOBONamespace>GAZ</oboInOwl:hasOBONamespace>
        <oboInOwl:id>GAZ:00118437</oboInOwl:id>
        <rdfs:label>Tonzang Township</rdfs:label>
    </owl:NamedIndividual>
    


    <!-- http://purl.obolibrary.org/obo/GAZ_00118438 -->

    <owl:NamedIndividual rdf:about="http://purl.obolibrary.org/obo/GAZ_00118438">
        <obo:RO_0001025 rdf:resource="http://purl.obolibrary.org/obo/GAZ_00025538"/>
        <obo:IAO_0000115>A populated place. A township of Falam District in the Chin State of Myanmar.</obo:IAO_0000115>
        <oboInOwl:hasOBONamespace>GAZ</oboInOwl:hasOBONamespace>
        <oboInOwl:id>GAZ:00118438</oboInOwl:id>
        <rdfs:label>Falam Township</rdfs:label>
    </owl:NamedIndividual>
    


    <!-- http://purl.obolibrary.org/obo/GAZ_00118439 -->

    <owl:NamedIndividual rdf:about="http://purl.obolibrary.org/obo/GAZ_00118439">
        <obo:RO_0001025 rdf:resource="http://purl.obolibrary.org/obo/GAZ_00025538"/>
        <obo:IAO_0000115>A populated place. A township of Falam District in the Chin State of Myanmar.</obo:IAO_0000115>
        <oboInOwl:hasOBONamespace>GAZ</oboInOwl:hasOBONamespace>
        <oboInOwl:id>GAZ:00118439</oboInOwl:id>
        <rdfs:label>Haka Township</rdfs:label>
    </owl:NamedIndividual>
    


    <!-- http://purl.obolibrary.org/obo/GAZ_00118440 -->

    <owl:NamedIndividual rdf:about="http://purl.obolibrary.org/obo/GAZ_00118440">
        <obo:RO_0001025 rdf:resource="http://purl.obolibrary.org/obo/GAZ_00025538"/>
        <obo:IAO_0000115>A populated place. A township of Falam District in the Chin State of Myanmar.</obo:IAO_0000115>
        <oboInOwl:hasOBONamespace>GAZ</oboInOwl:hasOBONamespace>
        <oboInOwl:id>GAZ:00118440</oboInOwl:id>
        <rdfs:label>Htantlang Township</rdfs:label>
    </owl:NamedIndividual>
    


    <!-- http://purl.obolibrary.org/obo/GAZ_00118441 -->

    <owl:NamedIndividual rdf:about="http://purl.obolibrary.org/obo/GAZ_00118441">
        <obo:RO_0001025 rdf:resource="http://purl.obolibrary.org/obo/GAZ_00025537"/>
        <obo:IAO_0000115>A populated place. A township of Mindat District in the Chin State of Myanmar.</obo:IAO_0000115>
        <oboInOwl:hasOBONamespace>GAZ</oboInOwl:hasOBONamespace>
        <oboInOwl:id>GAZ:00118441</oboInOwl:id>
        <rdfs:label>Kanpetlet Township</rdfs:label>
    </owl:NamedIndividual>
    


    <!-- http://purl.obolibrary.org/obo/GAZ_00118442 -->

    <owl:NamedIndividual rdf:about="http://purl.obolibrary.org/obo/GAZ_00118442">
        <obo:RO_0001025 rdf:resource="http://purl.obolibrary.org/obo/GAZ_00025537"/>
        <obo:IAO_0000115>A populated place. A township of Mindat District in the Chin State of Myanmar.</obo:IAO_0000115>
        <oboInOwl:hasOBONamespace>GAZ</oboInOwl:hasOBONamespace>
        <oboInOwl:id>GAZ:00118442</oboInOwl:id>
        <rdfs:label>Mindat Township</rdfs:label>
    </owl:NamedIndividual>
    


    <!-- http://purl.obolibrary.org/obo/GAZ_00118443 -->

    <owl:NamedIndividual rdf:about="http://purl.obolibrary.org/obo/GAZ_00118443">
        <obo:RO_0001025 rdf:resource="http://purl.obolibrary.org/obo/GAZ_00025537"/>
        <obo:IAO_0000115>A populated place. A township of Mindat District in the Chin State of Myanmar.</obo:IAO_0000115>
        <oboInOwl:hasOBONamespace>GAZ</oboInOwl:hasOBONamespace>
        <oboInOwl:id>GAZ:00118443</oboInOwl:id>
        <rdfs:label>Paletwa Township</rdfs:label>
    </owl:NamedIndividual>
    


    <!-- http://purl.obolibrary.org/obo/GAZ_00118444 -->

    <owl:NamedIndividual rdf:about="http://purl.obolibrary.org/obo/GAZ_00118444">
        <obo:RO_0001025 rdf:resource="http://purl.obolibrary.org/obo/GAZ_00025537"/>
        <obo:IAO_0000115>A populated place. A township of Mindat District in the Chin State of Myanmar.</obo:IAO_0000115>
        <oboInOwl:hasOBONamespace>GAZ</oboInOwl:hasOBONamespace>
        <oboInOwl:id>GAZ:00118444</oboInOwl:id>
        <rdfs:label>Matupi Township</rdfs:label>
    </owl:NamedIndividual>
    


    <!-- http://purl.obolibrary.org/obo/GAZ_00118445 -->

    <owl:NamedIndividual rdf:about="http://purl.obolibrary.org/obo/GAZ_00118445">
        <obo:RO_0001025 rdf:resource="http://purl.obolibrary.org/obo/GAZ_00025539"/>
        <obo:IAO_0000115>A populated place. A township (sub district) of Myitkyina District in Kachin State, Burma.</obo:IAO_0000115>
        <oboInOwl:hasOBONamespace>GAZ</oboInOwl:hasOBONamespace>
        <oboInOwl:id>GAZ:00118445</oboInOwl:id>
        <rdfs:label>Injangyang Township</rdfs:label>
    </owl:NamedIndividual>
    


    <!-- http://purl.obolibrary.org/obo/GAZ_00118446 -->

    <owl:NamedIndividual rdf:about="http://purl.obolibrary.org/obo/GAZ_00118446">
        <obo:RO_0001025 rdf:resource="http://purl.obolibrary.org/obo/GAZ_00025539"/>
        <obo:IAO_0000115>A populated place. A township (sub district) of Myitkyina District in Kachin State, Burma.</obo:IAO_0000115>
        <oboInOwl:hasOBONamespace>GAZ</oboInOwl:hasOBONamespace>
        <oboInOwl:id>GAZ:00118446</oboInOwl:id>
        <rdfs:label>Tanai Township</rdfs:label>
    </owl:NamedIndividual>
    


    <!-- http://purl.obolibrary.org/obo/GAZ_00118447 -->

    <owl:NamedIndividual rdf:about="http://purl.obolibrary.org/obo/GAZ_00118447">
        <obo:RO_0001025 rdf:resource="http://purl.obolibrary.org/obo/GAZ_00025539"/>
        <obo:IAO_0000115>A populated place. A township (sub district) of Myitkyina District in Kachin State, Burma.</obo:IAO_0000115>
        <oboInOwl:hasOBONamespace>GAZ</oboInOwl:hasOBONamespace>
        <oboInOwl:id>GAZ:00118447</oboInOwl:id>
        <rdfs:label>Sawlaw Township</rdfs:label>
    </owl:NamedIndividual>
    


    <!-- http://purl.obolibrary.org/obo/GAZ_00118448 -->

    <owl:NamedIndividual rdf:about="http://purl.obolibrary.org/obo/GAZ_00118448">
        <obo:RO_0001025 rdf:resource="http://purl.obolibrary.org/obo/GAZ_00025539"/>
        <obo:IAO_0000115>A populated place. A township (sub district) of Myitkyina District in Kachin State, Burma.</obo:IAO_0000115>
        <oboInOwl:hasOBONamespace>GAZ</oboInOwl:hasOBONamespace>
        <oboInOwl:id>GAZ:00118448</oboInOwl:id>
        <rdfs:label>Mongyaung Township</rdfs:label>
    </owl:NamedIndividual>
    


    <!-- http://purl.obolibrary.org/obo/GAZ_00118449 -->

    <owl:NamedIndividual rdf:about="http://purl.obolibrary.org/obo/GAZ_00118449">
        <obo:RO_0001025 rdf:resource="http://purl.obolibrary.org/obo/GAZ_00025539"/>
        <obo:IAO_0000115>A populated place. A township (sub district) of Myitkyina District in Kachin State, Burma.</obo:IAO_0000115>
        <oboInOwl:hasOBONamespace>GAZ</oboInOwl:hasOBONamespace>
        <oboInOwl:id>GAZ:00118449</oboInOwl:id>
        <rdfs:label>Hpakant Township</rdfs:label>
    </owl:NamedIndividual>
    


    <!-- http://purl.obolibrary.org/obo/GAZ_00118450 -->

    <owl:NamedIndividual rdf:about="http://purl.obolibrary.org/obo/GAZ_00118450">
        <obo:RO_0001025 rdf:resource="http://purl.obolibrary.org/obo/GAZ_00025539"/>
        <obo:IAO_0000115>A populated place. A township (sub district) of Myitkyina District in Kachin State, Burma.</obo:IAO_0000115>
        <oboInOwl:hasOBONamespace>GAZ</oboInOwl:hasOBONamespace>
        <oboInOwl:id>GAZ:00118450</oboInOwl:id>
        <rdfs:label>Mohnyin Township</rdfs:label>
    </owl:NamedIndividual>
    


    <!-- http://purl.obolibrary.org/obo/GAZ_00118451 -->

    <owl:NamedIndividual rdf:about="http://purl.obolibrary.org/obo/GAZ_00118451">
        <obo:RO_0001025 rdf:resource="http://purl.obolibrary.org/obo/GAZ_00025539"/>
        <obo:IAO_0000115>A populated place. A township (sub district) of Myitkyina District in Kachin State, Burma.</obo:IAO_0000115>
        <oboInOwl:hasOBONamespace>GAZ</oboInOwl:hasOBONamespace>
        <oboInOwl:id>GAZ:00118451</oboInOwl:id>
        <rdfs:label>Myitkyina Township</rdfs:label>
    </owl:NamedIndividual>
    


    <!-- http://purl.obolibrary.org/obo/GAZ_00118452 -->

    <owl:NamedIndividual rdf:about="http://purl.obolibrary.org/obo/GAZ_00118452">
        <obo:RO_0001025 rdf:resource="http://purl.obolibrary.org/obo/GAZ_00025539"/>
        <obo:IAO_0000115>A populated place. A township (sub district) of Myitkyina District in Kachin State, Burma.</obo:IAO_0000115>
        <oboInOwl:hasOBONamespace>GAZ</oboInOwl:hasOBONamespace>
        <oboInOwl:id>GAZ:00118452</oboInOwl:id>
        <rdfs:label>Waingmaw Township</rdfs:label>
    </owl:NamedIndividual>
    


    <!-- http://purl.obolibrary.org/obo/GAZ_00118453 -->

    <owl:NamedIndividual rdf:about="http://purl.obolibrary.org/obo/GAZ_00118453">
        <obo:RO_0001025 rdf:resource="http://purl.obolibrary.org/obo/GAZ_00025539"/>
        <obo:IAO_0000115>A populated place. A township (sub district) of Myitkyina District in Kachin State, Burma.</obo:IAO_0000115>
        <oboInOwl:hasOBONamespace>GAZ</oboInOwl:hasOBONamespace>
        <oboInOwl:id>GAZ:00118453</oboInOwl:id>
        <rdfs:label>Chipw Township</rdfs:label>
    </owl:NamedIndividual>
    


    <!-- http://purl.obolibrary.org/obo/GAZ_00118454 -->

    <owl:NamedIndividual rdf:about="http://purl.obolibrary.org/obo/GAZ_00118454">
        <obo:RO_0001025 rdf:resource="http://purl.obolibrary.org/obo/GAZ_00025541"/>
        <obo:IAO_0000115>A populated place. A township of Bhamo District in the Kachin State of Burma. The principal town is Bhamo.</obo:IAO_0000115>
        <oboInOwl:hasOBONamespace>GAZ</oboInOwl:hasOBONamespace>
        <oboInOwl:id>GAZ:00118454</oboInOwl:id>
        <rdfs:label>Bhamo Township</rdfs:label>
    </owl:NamedIndividual>
    


    <!-- http://purl.obolibrary.org/obo/GAZ_00118455 -->

    <owl:NamedIndividual rdf:about="http://purl.obolibrary.org/obo/GAZ_00118455">
        <obo:RO_0001025 rdf:resource="http://purl.obolibrary.org/obo/GAZ_00025541"/>
        <obo:IAO_0000115>A populated place. A township of Bhamo District in the Kachin State of Burma. The principal town is Shwegu.</obo:IAO_0000115>
        <oboInOwl:hasOBONamespace>GAZ</oboInOwl:hasOBONamespace>
        <oboInOwl:id>GAZ:00118455</oboInOwl:id>
        <rdfs:label>Shwegu Township</rdfs:label>
    </owl:NamedIndividual>
    


    <!-- http://purl.obolibrary.org/obo/GAZ_00118456 -->

    <owl:NamedIndividual rdf:about="http://purl.obolibrary.org/obo/GAZ_00118456">
        <obo:RO_0001025 rdf:resource="http://purl.obolibrary.org/obo/GAZ_00025541"/>
        <obo:IAO_0000115>A populated place. A township of Bhamo District in the Kachin State of Burma. The principal town is Mansi.</obo:IAO_0000115>
        <oboInOwl:hasOBONamespace>GAZ</oboInOwl:hasOBONamespace>
        <oboInOwl:id>GAZ:00118456</oboInOwl:id>
        <rdfs:label>Mansi Township</rdfs:label>
    </owl:NamedIndividual>
    


    <!-- http://purl.obolibrary.org/obo/GAZ_00118457 -->

    <owl:NamedIndividual rdf:about="http://purl.obolibrary.org/obo/GAZ_00118457">
        <obo:RO_0001025 rdf:resource="http://purl.obolibrary.org/obo/GAZ_00025541"/>
        <obo:IAO_0000115>A populated place. A township of Bhamo District in the Kachin State of Burma. The principal town is Momauk.</obo:IAO_0000115>
        <oboInOwl:hasOBONamespace>GAZ</oboInOwl:hasOBONamespace>
        <oboInOwl:id>GAZ:00118457</oboInOwl:id>
        <rdfs:label>Momauk Township</rdfs:label>
    </owl:NamedIndividual>
    


    <!-- http://purl.obolibrary.org/obo/GAZ_00118458 -->

    <owl:NamedIndividual rdf:about="http://purl.obolibrary.org/obo/GAZ_00118458">
        <obo:RO_0001025 rdf:resource="http://purl.obolibrary.org/obo/GAZ_00025540"/>
        <obo:IAO_0000115>A populated place. A township of Putao District in the Kachin State of Burma. The principal town is Machanbaw.</obo:IAO_0000115>
        <oboInOwl:hasOBONamespace>GAZ</oboInOwl:hasOBONamespace>
        <oboInOwl:id>GAZ:00118458</oboInOwl:id>
        <rdfs:label>Machanbaw Township</rdfs:label>
    </owl:NamedIndividual>
    


    <!-- http://purl.obolibrary.org/obo/GAZ_00118459 -->

    <owl:NamedIndividual rdf:about="http://purl.obolibrary.org/obo/GAZ_00118459">
        <obo:RO_0001025 rdf:resource="http://purl.obolibrary.org/obo/GAZ_00025540"/>
        <obo:IAO_0000115>A populated place. A township of Putao District in the Kachin State of Burma. The principal town is Putao.</obo:IAO_0000115>
        <oboInOwl:hasOBONamespace>GAZ</oboInOwl:hasOBONamespace>
        <oboInOwl:id>GAZ:00118459</oboInOwl:id>
        <rdfs:label>Putao Township</rdfs:label>
    </owl:NamedIndividual>
    


    <!-- http://purl.obolibrary.org/obo/GAZ_00118460 -->

    <owl:NamedIndividual rdf:about="http://purl.obolibrary.org/obo/GAZ_00118460">
        <obo:RO_0001025 rdf:resource="http://purl.obolibrary.org/obo/GAZ_00025540"/>
        <obo:IAO_0000115>A populated place. A township of Putao District in the Kachin State of Burma. The principal town is Nogmung.</obo:IAO_0000115>
        <oboInOwl:hasOBONamespace>GAZ</oboInOwl:hasOBONamespace>
        <oboInOwl:id>GAZ:00118460</oboInOwl:id>
        <rdfs:label>Nogmung Township</rdfs:label>
    </owl:NamedIndividual>
    


    <!-- http://purl.obolibrary.org/obo/GAZ_00118461 -->

    <owl:NamedIndividual rdf:about="http://purl.obolibrary.org/obo/GAZ_00118461">
        <obo:RO_0001025 rdf:resource="http://purl.obolibrary.org/obo/GAZ_00025540"/>
        <obo:IAO_0000115>A populated place. A township of Putao District in the Kachin State of Burma. The principal town is Kawnglanghpu.</obo:IAO_0000115>
        <oboInOwl:hasOBONamespace>GAZ</oboInOwl:hasOBONamespace>
        <oboInOwl:id>GAZ:00118461</oboInOwl:id>
        <rdfs:label>Kawnglanghpu Township</rdfs:label>
    </owl:NamedIndividual>
    


    <!-- http://purl.obolibrary.org/obo/GAZ_00118462 -->

    <owl:NamedIndividual rdf:about="http://purl.obolibrary.org/obo/GAZ_00118462">
        <obo:RO_0001025 rdf:resource="http://purl.obolibrary.org/obo/GAZ_00025540"/>
        <obo:IAO_0000115>A populated place. A township of Putao District in the Kachin State of Burma. The principal town is Sumprabum.</obo:IAO_0000115>
        <oboInOwl:hasOBONamespace>GAZ</oboInOwl:hasOBONamespace>
        <oboInOwl:id>GAZ:00118462</oboInOwl:id>
        <rdfs:label>Sumprabum Township</rdfs:label>
    </owl:NamedIndividual>
    


    <!-- http://purl.obolibrary.org/obo/GAZ_00118463 -->

    <owl:NamedIndividual rdf:about="http://purl.obolibrary.org/obo/GAZ_00118463">
        <obo:RO_0001025 rdf:resource="http://purl.obolibrary.org/obo/GAZ_00025542"/>
        <obo:IAO_0000115>A populated place. A township of Loikaw District in the eastern part of Kayah State in Myanmar.</obo:IAO_0000115>
        <oboInOwl:hasOBONamespace>GAZ</oboInOwl:hasOBONamespace>
        <oboInOwl:id>GAZ:00118463</oboInOwl:id>
        <rdfs:label>Demoso Township</rdfs:label>
    </owl:NamedIndividual>
    


    <!-- http://purl.obolibrary.org/obo/GAZ_00118464 -->

    <owl:NamedIndividual rdf:about="http://purl.obolibrary.org/obo/GAZ_00118464">
        <obo:RO_0001025 rdf:resource="http://purl.obolibrary.org/obo/GAZ_00025542"/>
        <obo:IAO_0000115>A populated place. A township of Loikaw District in the eastern part of Kayah State in Myanmar.</obo:IAO_0000115>
        <oboInOwl:hasOBONamespace>GAZ</oboInOwl:hasOBONamespace>
        <oboInOwl:id>GAZ:00118464</oboInOwl:id>
        <rdfs:label>Loikaw Township</rdfs:label>
    </owl:NamedIndividual>
    


    <!-- http://purl.obolibrary.org/obo/GAZ_00118465 -->

    <owl:NamedIndividual rdf:about="http://purl.obolibrary.org/obo/GAZ_00118465">
        <obo:RO_0001025 rdf:resource="http://purl.obolibrary.org/obo/GAZ_00025542"/>
        <obo:IAO_0000115>A populated place. A township of Loikaw District in the eastern part of Kayah State in Myanmar.</obo:IAO_0000115>
        <oboInOwl:hasOBONamespace>GAZ</oboInOwl:hasOBONamespace>
        <oboInOwl:id>GAZ:00118465</oboInOwl:id>
        <rdfs:label>Shadaw Township</rdfs:label>
    </owl:NamedIndividual>
    


    <!-- http://purl.obolibrary.org/obo/GAZ_00118466 -->

    <owl:NamedIndividual rdf:about="http://purl.obolibrary.org/obo/GAZ_00118466">
        <obo:RO_0001025 rdf:resource="http://purl.obolibrary.org/obo/GAZ_00025542"/>
        <obo:IAO_0000115>A populated place. A township of Loikaw District in the eastern part of Kayah State in Myanmar.</obo:IAO_0000115>
        <oboInOwl:hasOBONamespace>GAZ</oboInOwl:hasOBONamespace>
        <oboInOwl:id>GAZ:00118466</oboInOwl:id>
        <rdfs:label>Hpruso Township</rdfs:label>
    </owl:NamedIndividual>
    


    <!-- http://purl.obolibrary.org/obo/GAZ_00118467 -->

    <owl:NamedIndividual rdf:about="http://purl.obolibrary.org/obo/GAZ_00118467">
        <obo:RO_0001025 rdf:resource="http://purl.obolibrary.org/obo/GAZ_00025543"/>
        <obo:IAO_0000115>A populated place. A township of Bawlakhe District in the Kayah State of Myanmar. The principal town lies at Hpasaung.</obo:IAO_0000115>
        <oboInOwl:hasOBONamespace>GAZ</oboInOwl:hasOBONamespace>
        <oboInOwl:id>GAZ:00118467</oboInOwl:id>
        <rdfs:label>Hpasawng Township</rdfs:label>
    </owl:NamedIndividual>
    


    <!-- http://purl.obolibrary.org/obo/GAZ_00118468 -->

    <owl:NamedIndividual rdf:about="http://purl.obolibrary.org/obo/GAZ_00118468">
        <obo:RO_0001025 rdf:resource="http://purl.obolibrary.org/obo/GAZ_00025543"/>
        <obo:IAO_0000115>A populated place. A township of Bawlakhe District in the eastern part of Kayah State in Myanmar.</obo:IAO_0000115>
        <oboInOwl:hasOBONamespace>GAZ</oboInOwl:hasOBONamespace>
        <oboInOwl:id>GAZ:00118468</oboInOwl:id>
        <rdfs:label>Bawlakhe Township</rdfs:label>
    </owl:NamedIndividual>
    


    <!-- http://purl.obolibrary.org/obo/GAZ_00118469 -->

    <owl:NamedIndividual rdf:about="http://purl.obolibrary.org/obo/GAZ_00118469">
        <obo:RO_0001025 rdf:resource="http://purl.obolibrary.org/obo/GAZ_00025543"/>
        <obo:IAO_0000115>A populated place. A township of Bawlakhe District in the Kayah State of Myanmar. The principal town lies at Mese.</obo:IAO_0000115>
        <oboInOwl:hasOBONamespace>GAZ</oboInOwl:hasOBONamespace>
        <oboInOwl:id>GAZ:00118469</oboInOwl:id>
        <rdfs:label>Mese Township</rdfs:label>
    </owl:NamedIndividual>
    


    <!-- http://purl.obolibrary.org/obo/GAZ_00118470 -->

    <owl:NamedIndividual rdf:about="http://purl.obolibrary.org/obo/GAZ_00118470">
        <obo:RO_0001025 rdf:resource="http://purl.obolibrary.org/obo/GAZ_00025545"/>
        <obo:IAO_0000115>A populated place. A township of Kawkareik District in the Kayin State of Myanmar.</obo:IAO_0000115>
        <oboInOwl:hasOBONamespace>GAZ</oboInOwl:hasOBONamespace>
        <oboInOwl:id>GAZ:00118470</oboInOwl:id>
        <rdfs:label>Kawkareik Township</rdfs:label>
    </owl:NamedIndividual>
    


    <!-- http://purl.obolibrary.org/obo/GAZ_00118471 -->

    <owl:NamedIndividual rdf:about="http://purl.obolibrary.org/obo/GAZ_00118471">
        <obo:RO_0001025 rdf:resource="http://purl.obolibrary.org/obo/GAZ_00025545"/>
        <obo:IAO_0000115>A populated place. A township of Kawkareik District in the Kayin State of Myanmar.</obo:IAO_0000115>
        <oboInOwl:hasOBONamespace>GAZ</oboInOwl:hasOBONamespace>
        <oboInOwl:id>GAZ:00118471</oboInOwl:id>
        <rdfs:label>Kyain Seikgyi Township</rdfs:label>
    </owl:NamedIndividual>
    


    <!-- http://purl.obolibrary.org/obo/GAZ_00118472 -->

    <owl:NamedIndividual rdf:about="http://purl.obolibrary.org/obo/GAZ_00118472">
        <obo:RO_0001025 rdf:resource="http://purl.obolibrary.org/obo/GAZ_00025544"/>
        <obo:IAO_0000115>A populated place. A township of Hpa-an District in the Kayin State of Myanmar.</obo:IAO_0000115>
        <oboInOwl:hasOBONamespace>GAZ</oboInOwl:hasOBONamespace>
        <oboInOwl:id>GAZ:00118472</oboInOwl:id>
        <rdfs:label>Hlaignbwe Township</rdfs:label>
    </owl:NamedIndividual>
    


    <!-- http://purl.obolibrary.org/obo/GAZ_00118473 -->

    <owl:NamedIndividual rdf:about="http://purl.obolibrary.org/obo/GAZ_00118473">
        <obo:RO_0001025 rdf:resource="http://purl.obolibrary.org/obo/GAZ_00025544"/>
        <obo:IAO_0000115>A populated place. A township of Hpa-an District in the Kayin State of Myanmar.</obo:IAO_0000115>
        <oboInOwl:hasOBONamespace>GAZ</oboInOwl:hasOBONamespace>
        <oboInOwl:id>GAZ:00118473</oboInOwl:id>
        <rdfs:label>Hpa-an Township</rdfs:label>
    </owl:NamedIndividual>
    


    <!-- http://purl.obolibrary.org/obo/GAZ_00118474 -->

    <owl:NamedIndividual rdf:about="http://purl.obolibrary.org/obo/GAZ_00118474">
        <obo:RO_0001025 rdf:resource="http://purl.obolibrary.org/obo/GAZ_00025544"/>
        <obo:IAO_0000115>A populated place. A township of Hpa-an District in the Kayin State of Myanmar.</obo:IAO_0000115>
        <oboInOwl:hasOBONamespace>GAZ</oboInOwl:hasOBONamespace>
        <oboInOwl:id>GAZ:00118474</oboInOwl:id>
        <rdfs:label>Thandang Township</rdfs:label>
    </owl:NamedIndividual>
    


    <!-- http://purl.obolibrary.org/obo/GAZ_00118475 -->

    <owl:NamedIndividual rdf:about="http://purl.obolibrary.org/obo/GAZ_00118475">
        <obo:RO_0001025 rdf:resource="http://purl.obolibrary.org/obo/GAZ_00025544"/>
        <obo:IAO_0000115>A populated place. A township of Hpa-an District in the Kayin State of Myanmar.</obo:IAO_0000115>
        <oboInOwl:hasOBONamespace>GAZ</oboInOwl:hasOBONamespace>
        <oboInOwl:id>GAZ:00118475</oboInOwl:id>
        <rdfs:label>Hpapun Township</rdfs:label>
    </owl:NamedIndividual>
    


    <!-- http://purl.obolibrary.org/obo/GAZ_00118476 -->

    <owl:NamedIndividual rdf:about="http://purl.obolibrary.org/obo/GAZ_00118476">
        <obo:RO_0001025 rdf:resource="http://purl.obolibrary.org/obo/GAZ_00025546"/>
        <obo:IAO_0000115>A populated place. A township of Myawaddy District in the Kayin State of Myanmar.</obo:IAO_0000115>
        <oboInOwl:hasOBONamespace>GAZ</oboInOwl:hasOBONamespace>
        <oboInOwl:id>GAZ:00118476</oboInOwl:id>
        <rdfs:label>Myawaddy Township</rdfs:label>
    </owl:NamedIndividual>
    


    <!-- http://purl.obolibrary.org/obo/GAZ_00118477 -->

    <owl:NamedIndividual rdf:about="http://purl.obolibrary.org/obo/GAZ_00118477">
        <obo:RO_0001025 rdf:resource="http://purl.obolibrary.org/obo/GAZ_00025547"/>
        <obo:IAO_0000115>A populated place. A township of Mawlamyine District in the Mon State of Myanmar.</obo:IAO_0000115>
        <oboInOwl:hasOBONamespace>GAZ</oboInOwl:hasOBONamespace>
        <oboInOwl:id>GAZ:00118477</oboInOwl:id>
        <rdfs:label>Thanbyuzayat Township</rdfs:label>
    </owl:NamedIndividual>
    


    <!-- http://purl.obolibrary.org/obo/GAZ_00118478 -->

    <owl:NamedIndividual rdf:about="http://purl.obolibrary.org/obo/GAZ_00118478">
        <obo:RO_0001025 rdf:resource="http://purl.obolibrary.org/obo/GAZ_00025547"/>
        <obo:IAO_0000115>A populated place. A township of Mawlamyine District in the Mon State of Myanmar.</obo:IAO_0000115>
        <oboInOwl:hasOBONamespace>GAZ</oboInOwl:hasOBONamespace>
        <oboInOwl:id>GAZ:00118478</oboInOwl:id>
        <rdfs:label>Mawlamyine Township</rdfs:label>
    </owl:NamedIndividual>
    


    <!-- http://purl.obolibrary.org/obo/GAZ_00118479 -->

    <owl:NamedIndividual rdf:about="http://purl.obolibrary.org/obo/GAZ_00118479">
        <obo:RO_0001025 rdf:resource="http://purl.obolibrary.org/obo/GAZ_00025547"/>
        <obo:IAO_0000115>A populated place. A township of Mawlamyine District in the Mon State of Myanmar.</obo:IAO_0000115>
        <oboInOwl:hasOBONamespace>GAZ</oboInOwl:hasOBONamespace>
        <oboInOwl:id>GAZ:00118479</oboInOwl:id>
        <rdfs:label>Ye Township</rdfs:label>
    </owl:NamedIndividual>
    


    <!-- http://purl.obolibrary.org/obo/GAZ_00118480 -->

    <owl:NamedIndividual rdf:about="http://purl.obolibrary.org/obo/GAZ_00118480">
        <obo:RO_0001025 rdf:resource="http://purl.obolibrary.org/obo/GAZ_00025547"/>
        <obo:IAO_0000115>A populated place. A township of Mawlamyine District in the Mon State of Myanmar.</obo:IAO_0000115>
        <oboInOwl:hasOBONamespace>GAZ</oboInOwl:hasOBONamespace>
        <oboInOwl:id>GAZ:00118480</oboInOwl:id>
        <rdfs:label>Mudon Township</rdfs:label>
    </owl:NamedIndividual>
    


    <!-- http://purl.obolibrary.org/obo/GAZ_00118481 -->

    <owl:NamedIndividual rdf:about="http://purl.obolibrary.org/obo/GAZ_00118481">
        <obo:RO_0001025 rdf:resource="http://purl.obolibrary.org/obo/GAZ_00025547"/>
        <obo:IAO_0000115>A populated place. A township of Mawlamyine District in the Mon State of Myanmar.</obo:IAO_0000115>
        <oboInOwl:hasOBONamespace>GAZ</oboInOwl:hasOBONamespace>
        <oboInOwl:id>GAZ:00118481</oboInOwl:id>
        <rdfs:label>Kyaikmaraw Township</rdfs:label>
    </owl:NamedIndividual>
    


    <!-- http://purl.obolibrary.org/obo/GAZ_00118482 -->

    <owl:NamedIndividual rdf:about="http://purl.obolibrary.org/obo/GAZ_00118482">
        <obo:RO_0001025 rdf:resource="http://purl.obolibrary.org/obo/GAZ_00025547"/>
        <obo:IAO_0000115>A populated place. A township of Mawlamyine District in the Mon State of Myanmar.</obo:IAO_0000115>
        <oboInOwl:hasOBONamespace>GAZ</oboInOwl:hasOBONamespace>
        <oboInOwl:id>GAZ:00118482</oboInOwl:id>
        <rdfs:label>Chaungzon Township</rdfs:label>
    </owl:NamedIndividual>
    


    <!-- http://purl.obolibrary.org/obo/GAZ_00118483 -->

    <owl:NamedIndividual rdf:about="http://purl.obolibrary.org/obo/GAZ_00118483">
        <obo:RO_0001025 rdf:resource="http://purl.obolibrary.org/obo/GAZ_00025548"/>
        <obo:IAO_0000115>A populated place. A township of Thaton District in the Mon State of Myanmar.</obo:IAO_0000115>
        <oboInOwl:hasOBONamespace>GAZ</oboInOwl:hasOBONamespace>
        <oboInOwl:id>GAZ:00118483</oboInOwl:id>
        <rdfs:label>Paung Township</rdfs:label>
    </owl:NamedIndividual>
    


    <!-- http://purl.obolibrary.org/obo/GAZ_00118484 -->

    <owl:NamedIndividual rdf:about="http://purl.obolibrary.org/obo/GAZ_00118484">
        <obo:RO_0001025 rdf:resource="http://purl.obolibrary.org/obo/GAZ_00025548"/>
        <obo:IAO_0000115>A populated place. A township of Thaton District in the Mon State of Myanmar.</obo:IAO_0000115>
        <oboInOwl:hasOBONamespace>GAZ</oboInOwl:hasOBONamespace>
        <oboInOwl:id>GAZ:00118484</oboInOwl:id>
        <rdfs:label>Bilin Township</rdfs:label>
    </owl:NamedIndividual>
    


    <!-- http://purl.obolibrary.org/obo/GAZ_00118485 -->

    <owl:NamedIndividual rdf:about="http://purl.obolibrary.org/obo/GAZ_00118485">
        <obo:RO_0001025 rdf:resource="http://purl.obolibrary.org/obo/GAZ_00025548"/>
        <obo:IAO_0000115>A populated place. A township of Thaton District in the Mon State of Myanmar.</obo:IAO_0000115>
        <oboInOwl:hasOBONamespace>GAZ</oboInOwl:hasOBONamespace>
        <oboInOwl:id>GAZ:00118485</oboInOwl:id>
        <rdfs:label>Thaton Township</rdfs:label>
    </owl:NamedIndividual>
    


    <!-- http://purl.obolibrary.org/obo/GAZ_00118486 -->

    <owl:NamedIndividual rdf:about="http://purl.obolibrary.org/obo/GAZ_00118486">
        <obo:RO_0001025 rdf:resource="http://purl.obolibrary.org/obo/GAZ_00025548"/>
        <obo:IAO_0000115>A populated place. A township of Thaton District in the Mon State of Myanmar.</obo:IAO_0000115>
        <oboInOwl:hasOBONamespace>GAZ</oboInOwl:hasOBONamespace>
        <oboInOwl:id>GAZ:00118486</oboInOwl:id>
        <rdfs:label>Kyaikto Township</rdfs:label>
    </owl:NamedIndividual>
    


    <!-- http://purl.obolibrary.org/obo/GAZ_00118487 -->

    <owl:NamedIndividual rdf:about="http://purl.obolibrary.org/obo/GAZ_00118487">
        <obo:RO_0001025 rdf:resource="http://purl.obolibrary.org/obo/GAZ_00025552"/>
        <obo:IAO_0000115>A populated place. A township of Sittwe District in the Rakhine State of Myanmar. The principal town is Sittwe.</obo:IAO_0000115>
        <oboInOwl:hasOBONamespace>GAZ</oboInOwl:hasOBONamespace>
        <oboInOwl:id>GAZ:00118487</oboInOwl:id>
        <rdfs:label>Sittwe Township</rdfs:label>
    </owl:NamedIndividual>
    


    <!-- http://purl.obolibrary.org/obo/GAZ_00118488 -->

    <owl:NamedIndividual rdf:about="http://purl.obolibrary.org/obo/GAZ_00118488">
        <obo:RO_0001025 rdf:resource="http://purl.obolibrary.org/obo/GAZ_00025552"/>
        <obo:IAO_0000115>A populated place. A township of Sittwe District in the Rakhine State of Myanmar. The principal town is Mrauk-U.</obo:IAO_0000115>
        <oboInOwl:hasOBONamespace>GAZ</oboInOwl:hasOBONamespace>
        <oboInOwl:id>GAZ:00118488</oboInOwl:id>
        <rdfs:label>Mrauk-U Township</rdfs:label>
    </owl:NamedIndividual>
    


    <!-- http://purl.obolibrary.org/obo/GAZ_00118489 -->

    <owl:NamedIndividual rdf:about="http://purl.obolibrary.org/obo/GAZ_00118489">
        <obo:RO_0001025 rdf:resource="http://purl.obolibrary.org/obo/GAZ_00025552"/>
        <obo:IAO_0000115>A populated place. A township of Sittwe District in the Rakhine State of Myanmar. The principal town is Rathedaung.</obo:IAO_0000115>
        <oboInOwl:hasOBONamespace>GAZ</oboInOwl:hasOBONamespace>
        <oboInOwl:id>GAZ:00118489</oboInOwl:id>
        <rdfs:label>Rathedaung Township</rdfs:label>
    </owl:NamedIndividual>
    


    <!-- http://purl.obolibrary.org/obo/GAZ_00118490 -->

    <owl:NamedIndividual rdf:about="http://purl.obolibrary.org/obo/GAZ_00118490">
        <obo:RO_0001025 rdf:resource="http://purl.obolibrary.org/obo/GAZ_00025552"/>
        <obo:IAO_0000115>A populated place. A township of Sittwe District in the Rakhine State of Myanmar. The principal town is Ponnagyun.</obo:IAO_0000115>
        <oboInOwl:hasOBONamespace>GAZ</oboInOwl:hasOBONamespace>
        <oboInOwl:id>GAZ:00118490</oboInOwl:id>
        <rdfs:label>Ponnagyun Township</rdfs:label>
    </owl:NamedIndividual>
    


    <!-- http://purl.obolibrary.org/obo/GAZ_00118491 -->

    <owl:NamedIndividual rdf:about="http://purl.obolibrary.org/obo/GAZ_00118491">
        <obo:RO_0001025 rdf:resource="http://purl.obolibrary.org/obo/GAZ_00025552"/>
        <obo:IAO_0000115>A populated place. A township of Sittwe District in the Rakhine State of Myanmar. The principal town is Myebon.</obo:IAO_0000115>
        <oboInOwl:hasOBONamespace>GAZ</oboInOwl:hasOBONamespace>
        <oboInOwl:id>GAZ:00118491</oboInOwl:id>
        <rdfs:label>Myebon Township</rdfs:label>
    </owl:NamedIndividual>
    


    <!-- http://purl.obolibrary.org/obo/GAZ_00118492 -->

    <owl:NamedIndividual rdf:about="http://purl.obolibrary.org/obo/GAZ_00118492">
        <obo:RO_0001025 rdf:resource="http://purl.obolibrary.org/obo/GAZ_00025552"/>
        <obo:IAO_0000115>A populated place. A township of Sittwe District in the Rakhine State of Myanmar. The principal town is Kyauktaw.</obo:IAO_0000115>
        <oboInOwl:hasOBONamespace>GAZ</oboInOwl:hasOBONamespace>
        <oboInOwl:id>GAZ:00118492</oboInOwl:id>
        <rdfs:label>Kyauktaw Township</rdfs:label>
    </owl:NamedIndividual>
    


    <!-- http://purl.obolibrary.org/obo/GAZ_00118493 -->

    <owl:NamedIndividual rdf:about="http://purl.obolibrary.org/obo/GAZ_00118493">
        <obo:RO_0001025 rdf:resource="http://purl.obolibrary.org/obo/GAZ_00025552"/>
        <obo:IAO_0000115>A populated place. A township of Sittwe District in the Rakhine State of Myanmar. The principal town is Minbya.</obo:IAO_0000115>
        <oboInOwl:hasOBONamespace>GAZ</oboInOwl:hasOBONamespace>
        <oboInOwl:id>GAZ:00118493</oboInOwl:id>
        <rdfs:label>Minbya Township</rdfs:label>
    </owl:NamedIndividual>
    


    <!-- http://purl.obolibrary.org/obo/GAZ_00118494 -->

    <owl:NamedIndividual rdf:about="http://purl.obolibrary.org/obo/GAZ_00118494">
        <obo:RO_0001025 rdf:resource="http://purl.obolibrary.org/obo/GAZ_00025552"/>
        <obo:IAO_0000115>A populated place. A township of Sittwe District in the Rakhine State of Myanmar. The principal town is Pauktaw.</obo:IAO_0000115>
        <oboInOwl:hasOBONamespace>GAZ</oboInOwl:hasOBONamespace>
        <oboInOwl:id>GAZ:00118494</oboInOwl:id>
        <rdfs:label>Pauktaw Township</rdfs:label>
    </owl:NamedIndividual>
    


    <!-- http://purl.obolibrary.org/obo/GAZ_00118495 -->

    <owl:NamedIndividual rdf:about="http://purl.obolibrary.org/obo/GAZ_00118495">
        <obo:RO_0001025 rdf:resource="http://purl.obolibrary.org/obo/GAZ_00025551"/>
        <obo:IAO_0000115>A populated place. A township of Maungdaw District in the Rakhine State of Myanmar. The principal town is Maungdaw.</obo:IAO_0000115>
        <oboInOwl:hasOBONamespace>GAZ</oboInOwl:hasOBONamespace>
        <oboInOwl:id>GAZ:00118495</oboInOwl:id>
        <rdfs:label>Maungdaw Township</rdfs:label>
    </owl:NamedIndividual>
    


    <!-- http://purl.obolibrary.org/obo/GAZ_00118496 -->

    <owl:NamedIndividual rdf:about="http://purl.obolibrary.org/obo/GAZ_00118496">
        <obo:RO_0001025 rdf:resource="http://purl.obolibrary.org/obo/GAZ_00025551"/>
        <obo:IAO_0000115>A populated place. A township of Maungdaw District in the Rakhine State of Myanmar. The principal town is Buthidaung.</obo:IAO_0000115>
        <oboInOwl:hasOBONamespace>GAZ</oboInOwl:hasOBONamespace>
        <oboInOwl:id>GAZ:00118496</oboInOwl:id>
        <rdfs:label>Buthidaung Township</rdfs:label>
    </owl:NamedIndividual>
    


    <!-- http://purl.obolibrary.org/obo/GAZ_00118497 -->

    <owl:NamedIndividual rdf:about="http://purl.obolibrary.org/obo/GAZ_00118497">
        <obo:RO_0001025 rdf:resource="http://purl.obolibrary.org/obo/GAZ_00045834"/>
        <obo:IAO_0000115>A populated place. A township of Kyaukpyu District in the Rakhine State of Myanmar. The principal town is Ramree.</obo:IAO_0000115>
        <oboInOwl:hasOBONamespace>GAZ</oboInOwl:hasOBONamespace>
        <oboInOwl:id>GAZ:00118497</oboInOwl:id>
        <rdfs:label>Ramree Township</rdfs:label>
    </owl:NamedIndividual>
    


    <!-- http://purl.obolibrary.org/obo/GAZ_00118498 -->

    <owl:NamedIndividual rdf:about="http://purl.obolibrary.org/obo/GAZ_00118498">
        <obo:RO_0001025 rdf:resource="http://purl.obolibrary.org/obo/GAZ_00025550"/>
        <obo:IAO_0000115>A populated place. A township of Kyaukpyu District in the Rakhine State of Myanmar. The principal town is Kyaukpyu.</obo:IAO_0000115>
        <oboInOwl:hasOBONamespace>GAZ</oboInOwl:hasOBONamespace>
        <oboInOwl:id>GAZ:00118498</oboInOwl:id>
        <rdfs:label>Kyaukpyu Township</rdfs:label>
    </owl:NamedIndividual>
    


    <!-- http://purl.obolibrary.org/obo/GAZ_00118499 -->

    <owl:NamedIndividual rdf:about="http://purl.obolibrary.org/obo/GAZ_00118499">
        <obo:RO_0001025 rdf:resource="http://purl.obolibrary.org/obo/GAZ_00025550"/>
        <obo:IAO_0000115>A populated place. A township of Kyaukpyu District in the Rakhine State of Myanmar. The principal town is Ann.</obo:IAO_0000115>
        <oboInOwl:hasOBONamespace>GAZ</oboInOwl:hasOBONamespace>
        <oboInOwl:id>GAZ:00118499</oboInOwl:id>
        <rdfs:label>Ann Township</rdfs:label>
    </owl:NamedIndividual>
    


    <!-- http://purl.obolibrary.org/obo/GAZ_00118500 -->

    <owl:NamedIndividual rdf:about="http://purl.obolibrary.org/obo/GAZ_00118500">
        <obo:RO_0001025 rdf:resource="http://purl.obolibrary.org/obo/GAZ_00046071"/>
        <obo:IAO_0000115>A populated place. A township of Kyaukpyu District in the Rakhine State of Myanmar. The principal town is Manaung.</obo:IAO_0000115>
        <oboInOwl:hasOBONamespace>GAZ</oboInOwl:hasOBONamespace>
        <oboInOwl:id>GAZ:00118500</oboInOwl:id>
        <rdfs:label>Manaung Township</rdfs:label>
    </owl:NamedIndividual>
    


    <!-- http://purl.obolibrary.org/obo/GAZ_00118501 -->

    <owl:NamedIndividual rdf:about="http://purl.obolibrary.org/obo/GAZ_00118501">
        <obo:RO_0001025 rdf:resource="http://purl.obolibrary.org/obo/GAZ_00025553"/>
        <obo:IAO_0000115>A populated place. A township of Thandwe District in the Rakhine State of Myanmar. The principal town is Thandwe.</obo:IAO_0000115>
        <oboInOwl:hasOBONamespace>GAZ</oboInOwl:hasOBONamespace>
        <oboInOwl:id>GAZ:00118501</oboInOwl:id>
        <rdfs:label>Thandwe Township</rdfs:label>
    </owl:NamedIndividual>
    


    <!-- http://purl.obolibrary.org/obo/GAZ_00118502 -->

    <owl:NamedIndividual rdf:about="http://purl.obolibrary.org/obo/GAZ_00118502">
        <obo:RO_0001025 rdf:resource="http://purl.obolibrary.org/obo/GAZ_00025553"/>
        <obo:IAO_0000115>A populated place. A township of Thandwe District in the Rakhine State of Myanmar. The principal town is Toungup.</obo:IAO_0000115>
        <oboInOwl:hasOBONamespace>GAZ</oboInOwl:hasOBONamespace>
        <oboInOwl:id>GAZ:00118502</oboInOwl:id>
        <rdfs:label>Toungup Township</rdfs:label>
    </owl:NamedIndividual>
    


    <!-- http://purl.obolibrary.org/obo/GAZ_00118503 -->

    <owl:NamedIndividual rdf:about="http://purl.obolibrary.org/obo/GAZ_00118503">
        <obo:RO_0001025 rdf:resource="http://purl.obolibrary.org/obo/GAZ_00025553"/>
        <obo:IAO_0000115>A populated place. A township of Thandwe District in the Rakhine State of Myanmar. The principal town is Gaw.</obo:IAO_0000115>
        <oboInOwl:hasOBONamespace>GAZ</oboInOwl:hasOBONamespace>
        <oboInOwl:id>GAZ:00118503</oboInOwl:id>
        <rdfs:label>Gaw Township</rdfs:label>
    </owl:NamedIndividual>
    


    <!-- http://purl.obolibrary.org/obo/GAZ_00118504 -->

    <owl:NamedIndividual rdf:about="http://purl.obolibrary.org/obo/GAZ_00118504">
        <obo:RO_0001025 rdf:resource="http://purl.obolibrary.org/obo/GAZ_00025554"/>
        <obo:IAO_0000115>A populated place. A township of Kengtong District in the Shan State of Burma. The principal town is Mong Khet.</obo:IAO_0000115>
        <oboInOwl:hasOBONamespace>GAZ</oboInOwl:hasOBONamespace>
        <oboInOwl:id>GAZ:00118504</oboInOwl:id>
        <rdfs:label>Mong Khet Township</rdfs:label>
    </owl:NamedIndividual>
    


    <!-- http://purl.obolibrary.org/obo/GAZ_00118505 -->

    <owl:NamedIndividual rdf:about="http://purl.obolibrary.org/obo/GAZ_00118505">
        <obo:RO_0001025 rdf:resource="http://purl.obolibrary.org/obo/GAZ_00025554"/>
        <obo:IAO_0000115>A populated place. A township of Kengtung District in the Shan State of Burma. The principal town is Kengtung.</obo:IAO_0000115>
        <oboInOwl:hasOBONamespace>GAZ</oboInOwl:hasOBONamespace>
        <oboInOwl:id>GAZ:00118505</oboInOwl:id>
        <rdfs:label>Kengtung Township</rdfs:label>
    </owl:NamedIndividual>
    


    <!-- http://purl.obolibrary.org/obo/GAZ_00118506 -->

    <owl:NamedIndividual rdf:about="http://purl.obolibrary.org/obo/GAZ_00118506">
        <obo:RO_0001025 rdf:resource="http://purl.obolibrary.org/obo/GAZ_00025554"/>
        <obo:IAO_0000115>A populated place. A township of Kengtong District in the Shan State of Burma. The principal town is Mong Yang.</obo:IAO_0000115>
        <oboInOwl:hasOBONamespace>GAZ</oboInOwl:hasOBONamespace>
        <oboInOwl:id>GAZ:00118506</oboInOwl:id>
        <rdfs:label>Mong Yang Township</rdfs:label>
    </owl:NamedIndividual>
    


    <!-- http://purl.obolibrary.org/obo/GAZ_00118507 -->

    <owl:NamedIndividual rdf:about="http://purl.obolibrary.org/obo/GAZ_00118507">
        <obo:RO_0001025 rdf:resource="http://purl.obolibrary.org/obo/GAZ_00025555"/>
        <obo:IAO_0000115>A populated place. A township of Kunlong District in the Shan State of Burma. The principal town is Kunlong.</obo:IAO_0000115>
        <oboInOwl:hasOBONamespace>GAZ</oboInOwl:hasOBONamespace>
        <oboInOwl:id>GAZ:00118507</oboInOwl:id>
        <rdfs:label>Kunlong Township</rdfs:label>
    </owl:NamedIndividual>
    


    <!-- http://purl.obolibrary.org/obo/GAZ_00118508 -->

    <owl:NamedIndividual rdf:about="http://purl.obolibrary.org/obo/GAZ_00118508">
        <obo:RO_0001025 rdf:resource="http://purl.obolibrary.org/obo/GAZ_00025555"/>
        <obo:IAO_0000115>A populated place. A township of Kunlong District in the Shan State of Burma. The principal town is Hopang.</obo:IAO_0000115>
        <oboInOwl:hasOBONamespace>GAZ</oboInOwl:hasOBONamespace>
        <oboInOwl:id>GAZ:00118508</oboInOwl:id>
        <rdfs:label>Hopang Township</rdfs:label>
    </owl:NamedIndividual>
    


    <!-- http://purl.obolibrary.org/obo/GAZ_00118509 -->

    <owl:NamedIndividual rdf:about="http://purl.obolibrary.org/obo/GAZ_00118509">
        <obo:RO_0001025 rdf:resource="http://purl.obolibrary.org/obo/GAZ_00025556"/>
        <obo:IAO_0000115>A populated place. A township of Kyaukme District in the Shan State of eastern Burma. The principal town is Hsipaw.</obo:IAO_0000115>
        <oboInOwl:hasOBONamespace>GAZ</oboInOwl:hasOBONamespace>
        <oboInOwl:id>GAZ:00118509</oboInOwl:id>
        <rdfs:label>Hsipaw Township</rdfs:label>
    </owl:NamedIndividual>
    


    <!-- http://purl.obolibrary.org/obo/GAZ_00118510 -->

    <owl:NamedIndividual rdf:about="http://purl.obolibrary.org/obo/GAZ_00118510">
        <obo:RO_0001025 rdf:resource="http://purl.obolibrary.org/obo/GAZ_00025556"/>
        <obo:IAO_0000115>A populated place. A township of Kyaukme District in the Shan State of eastern Burma. The principal town is Kyaukme.</obo:IAO_0000115>
        <oboInOwl:hasOBONamespace>GAZ</oboInOwl:hasOBONamespace>
        <oboInOwl:id>GAZ:00118510</oboInOwl:id>
        <rdfs:label>Kyaukme Township</rdfs:label>
    </owl:NamedIndividual>
    


    <!-- http://purl.obolibrary.org/obo/GAZ_00118511 -->

    <owl:NamedIndividual rdf:about="http://purl.obolibrary.org/obo/GAZ_00118511">
        <obo:RO_0001025 rdf:resource="http://purl.obolibrary.org/obo/GAZ_00025556"/>
        <obo:IAO_0000115>A populated place. A township of Kyaukme District in the Shan State of eastern Burma. The principal town is Mabein.</obo:IAO_0000115>
        <oboInOwl:hasOBONamespace>GAZ</oboInOwl:hasOBONamespace>
        <oboInOwl:id>GAZ:00118511</oboInOwl:id>
        <rdfs:label>Mabein Township</rdfs:label>
    </owl:NamedIndividual>
    


    <!-- http://purl.obolibrary.org/obo/GAZ_00118512 -->

    <owl:NamedIndividual rdf:about="http://purl.obolibrary.org/obo/GAZ_00118512">
        <obo:RO_0001025 rdf:resource="http://purl.obolibrary.org/obo/GAZ_00025556"/>
        <obo:IAO_0000115>A populated place. A township of Kyaukme District in the Shan State of Burma. The principal town is Mantong.</obo:IAO_0000115>
        <oboInOwl:hasOBONamespace>GAZ</oboInOwl:hasOBONamespace>
        <oboInOwl:id>GAZ:00118512</oboInOwl:id>
        <rdfs:label>Mantong Township</rdfs:label>
    </owl:NamedIndividual>
    


    <!-- http://purl.obolibrary.org/obo/GAZ_00118513 -->

    <owl:NamedIndividual rdf:about="http://purl.obolibrary.org/obo/GAZ_00118513">
        <obo:RO_0001025 rdf:resource="http://purl.obolibrary.org/obo/GAZ_00025556"/>
        <obo:IAO_0000115>A populated place. A township of Kyaukme District in the Shan State of eastern Burma. The principal town is Mongmit.</obo:IAO_0000115>
        <oboInOwl:hasOBONamespace>GAZ</oboInOwl:hasOBONamespace>
        <oboInOwl:id>GAZ:00118513</oboInOwl:id>
        <rdfs:label>Mongmit Township</rdfs:label>
    </owl:NamedIndividual>
    


    <!-- http://purl.obolibrary.org/obo/GAZ_00118514 -->

    <owl:NamedIndividual rdf:about="http://purl.obolibrary.org/obo/GAZ_00118514">
        <obo:RO_0001025 rdf:resource="http://purl.obolibrary.org/obo/GAZ_00025556"/>
        <obo:IAO_0000115>A populated place. A township of Kyaukme District in the Shan State of eastern Burma. The principal town is Nawnghkio.</obo:IAO_0000115>
        <oboInOwl:hasOBONamespace>GAZ</oboInOwl:hasOBONamespace>
        <oboInOwl:id>GAZ:00118514</oboInOwl:id>
        <rdfs:label>Nawnghkio Township</rdfs:label>
    </owl:NamedIndividual>
    


    <!-- http://purl.obolibrary.org/obo/GAZ_00118515 -->

    <owl:NamedIndividual rdf:about="http://purl.obolibrary.org/obo/GAZ_00118515">
        <obo:RO_0001025 rdf:resource="http://purl.obolibrary.org/obo/GAZ_00025556"/>
        <obo:IAO_0000115>A populated place. A township of Kyaukme District in the Shan State of eastern Burma. The principal town is Namtu.</obo:IAO_0000115>
        <oboInOwl:hasOBONamespace>GAZ</oboInOwl:hasOBONamespace>
        <oboInOwl:id>GAZ:00118515</oboInOwl:id>
        <rdfs:label>Namtu Township</rdfs:label>
    </owl:NamedIndividual>
    


    <!-- http://purl.obolibrary.org/obo/GAZ_00118516 -->

    <owl:NamedIndividual rdf:about="http://purl.obolibrary.org/obo/GAZ_00118516">
        <obo:RO_0001025 rdf:resource="http://purl.obolibrary.org/obo/GAZ_00025556"/>
        <obo:IAO_0000115>A populated place. A township of Kyaukme District in the Shan State of eastern Burma. The principal town is Namhsan.</obo:IAO_0000115>
        <oboInOwl:hasOBONamespace>GAZ</oboInOwl:hasOBONamespace>
        <oboInOwl:id>GAZ:00118516</oboInOwl:id>
        <rdfs:label>Namhsan Township</rdfs:label>
    </owl:NamedIndividual>
    


    <!-- http://purl.obolibrary.org/obo/GAZ_00118517 -->

    <owl:NamedIndividual rdf:about="http://purl.obolibrary.org/obo/GAZ_00118517">
        <obo:RO_0001025 rdf:resource="http://purl.obolibrary.org/obo/GAZ_00025558"/>
        <obo:IAO_0000115>A populated place. A township of Laukkaing District in the Shan State of Burma. The principal town is Laukkaing.</obo:IAO_0000115>
        <oboInOwl:hasOBONamespace>GAZ</oboInOwl:hasOBONamespace>
        <oboInOwl:id>GAZ:00118517</oboInOwl:id>
        <rdfs:label>Laukkaing Township</rdfs:label>
    </owl:NamedIndividual>
    


    <!-- http://purl.obolibrary.org/obo/GAZ_00118518 -->

    <owl:NamedIndividual rdf:about="http://purl.obolibrary.org/obo/GAZ_00118518">
        <obo:RO_0001025 rdf:resource="http://purl.obolibrary.org/obo/GAZ_00025562"/>
        <obo:IAO_0000115>A populated place. A township of Mu Se District in the Shan State of eastern Burma. The principal town is Mu Se.</obo:IAO_0000115>
        <oboInOwl:hasOBONamespace>GAZ</oboInOwl:hasOBONamespace>
        <oboInOwl:id>GAZ:00118518</oboInOwl:id>
        <rdfs:label>Mu Se Township</rdfs:label>
    </owl:NamedIndividual>
    


    <!-- http://purl.obolibrary.org/obo/GAZ_00118519 -->

    <owl:NamedIndividual rdf:about="http://purl.obolibrary.org/obo/GAZ_00118519">
        <obo:RO_0001025 rdf:resource="http://purl.obolibrary.org/obo/GAZ_00025562"/>
        <obo:IAO_0000115>A populated place. A township of Mu Se District in the Shan State of eastern Burma. The principal town is Nanhkan.</obo:IAO_0000115>
        <oboInOwl:hasOBONamespace>GAZ</oboInOwl:hasOBONamespace>
        <oboInOwl:id>GAZ:00118519</oboInOwl:id>
        <rdfs:label>Nanhkan Township</rdfs:label>
    </owl:NamedIndividual>
    


    <!-- http://purl.obolibrary.org/obo/GAZ_00118520 -->

    <owl:NamedIndividual rdf:about="http://purl.obolibrary.org/obo/GAZ_00118520">
        <obo:RO_0001025 rdf:resource="http://purl.obolibrary.org/obo/GAZ_00025562"/>
        <obo:IAO_0000115>A populated place. A township of Muse District in the Shan State of eastern Burma. The principal town is Kutkai.</obo:IAO_0000115>
        <oboInOwl:hasOBONamespace>GAZ</oboInOwl:hasOBONamespace>
        <oboInOwl:id>GAZ:00118520</oboInOwl:id>
        <rdfs:label>Kutkai Township</rdfs:label>
    </owl:NamedIndividual>
    


    <!-- http://purl.obolibrary.org/obo/GAZ_00118521 -->

    <owl:NamedIndividual rdf:about="http://purl.obolibrary.org/obo/GAZ_00118521">
        <obo:RO_0001025 rdf:resource="http://purl.obolibrary.org/obo/GAZ_00025564"/>
        <obo:IAO_0000115>A populated place. A township of Taunggyi District in the Shan State of Myanmar. The principal town is Nyaungshwe.</obo:IAO_0000115>
        <oboInOwl:hasOBONamespace>GAZ</oboInOwl:hasOBONamespace>
        <oboInOwl:id>GAZ:00118521</oboInOwl:id>
        <rdfs:label>Nyaungshwe Township</rdfs:label>
    </owl:NamedIndividual>
    


    <!-- http://purl.obolibrary.org/obo/GAZ_00118522 -->

    <owl:NamedIndividual rdf:about="http://purl.obolibrary.org/obo/GAZ_00118522">
        <obo:RO_0001025 rdf:resource="http://purl.obolibrary.org/obo/GAZ_00025564"/>
        <obo:IAO_0000115>A populated place. A township of Taunggyi District in the Shan State of Myanmar. The principal town is Taunggyi.</obo:IAO_0000115>
        <oboInOwl:hasOBONamespace>GAZ</oboInOwl:hasOBONamespace>
        <oboInOwl:id>GAZ:00118522</oboInOwl:id>
        <rdfs:label>Taunggyi Township</rdfs:label>
    </owl:NamedIndividual>
    


    <!-- http://purl.obolibrary.org/obo/GAZ_00118523 -->

    <owl:NamedIndividual rdf:about="http://purl.obolibrary.org/obo/GAZ_00118523">
        <obo:RO_0001025 rdf:resource="http://purl.obolibrary.org/obo/GAZ_00025564"/>
        <obo:IAO_0000115>A populated place. A township of Taunggyi District in the Shan State of Myanmar. The principal town is Pekon.</obo:IAO_0000115>
        <oboInOwl:hasOBONamespace>GAZ</oboInOwl:hasOBONamespace>
        <oboInOwl:id>GAZ:00118523</oboInOwl:id>
        <rdfs:label>Pekon Township</rdfs:label>
    </owl:NamedIndividual>
    


    <!-- http://purl.obolibrary.org/obo/GAZ_00118524 -->

    <owl:NamedIndividual rdf:about="http://purl.obolibrary.org/obo/GAZ_00118524">
        <obo:RO_0001025 rdf:resource="http://purl.obolibrary.org/obo/GAZ_00025564"/>
        <obo:IAO_0000115>A populated place. A township of Taunggyi District in the Shan State of Myanmar. The principal town is Pinlaung.</obo:IAO_0000115>
        <oboInOwl:hasOBONamespace>GAZ</oboInOwl:hasOBONamespace>
        <oboInOwl:id>GAZ:00118524</oboInOwl:id>
        <rdfs:label>Pinlaung Township</rdfs:label>
    </owl:NamedIndividual>
    


    <!-- http://purl.obolibrary.org/obo/GAZ_00118525 -->

    <owl:NamedIndividual rdf:about="http://purl.obolibrary.org/obo/GAZ_00118525">
        <obo:RO_0001025 rdf:resource="http://purl.obolibrary.org/obo/GAZ_00025564"/>
        <obo:IAO_0000115>A populated place. A township of Taunggyi District in the Shan State of Myanmar. The principal town is Lawksawk. Lawksawk Township is bounded on the north by the townships of Nawnghkio, Kyaukme, and Hsipaw; on the east by Mong Kung and Hopong; on the south by Taunggyi, Kalaw, and Pingdaya; and on the west by Ywangan.</obo:IAO_0000115>
        <oboInOwl:hasOBONamespace>GAZ</oboInOwl:hasOBONamespace>
        <oboInOwl:id>GAZ:00118525</oboInOwl:id>
        <rdfs:label>Lawksawk Township</rdfs:label>
    </owl:NamedIndividual>
    


    <!-- http://purl.obolibrary.org/obo/GAZ_00118526 -->

    <owl:NamedIndividual rdf:about="http://purl.obolibrary.org/obo/GAZ_00118526">
        <obo:RO_0001025 rdf:resource="http://purl.obolibrary.org/obo/GAZ_00025564"/>
        <obo:IAO_0000115>A populated place. A township of Taunggyi District in the Shan State of Myanmar. The principal town is Pindaya.</obo:IAO_0000115>
        <oboInOwl:hasOBONamespace>GAZ</oboInOwl:hasOBONamespace>
        <oboInOwl:id>GAZ:00118526</oboInOwl:id>
        <rdfs:label>Pingdaya Township</rdfs:label>
    </owl:NamedIndividual>
    


    <!-- http://purl.obolibrary.org/obo/GAZ_00118527 -->

    <owl:NamedIndividual rdf:about="http://purl.obolibrary.org/obo/GAZ_00118527">
        <obo:RO_0001025 rdf:resource="http://purl.obolibrary.org/obo/GAZ_00025564"/>
        <obo:IAO_0000115>A populated place. A township of Taunggyi District in the Shan State of Myanmar. The principal town is Hsi Hseng.</obo:IAO_0000115>
        <oboInOwl:hasOBONamespace>GAZ</oboInOwl:hasOBONamespace>
        <oboInOwl:id>GAZ:00118527</oboInOwl:id>
        <rdfs:label>Hsi Hseng Township</rdfs:label>
    </owl:NamedIndividual>
    


    <!-- http://purl.obolibrary.org/obo/GAZ_00118528 -->

    <owl:NamedIndividual rdf:about="http://purl.obolibrary.org/obo/GAZ_00118528">
        <obo:RO_0001025 rdf:resource="http://purl.obolibrary.org/obo/GAZ_00025564"/>
        <obo:IAO_0000115>A populated place. A township of Taunggyi District in the Shan State of Myanmar. The principal town is Kalaw. This township has two towns: Kalaw and Aungban.</obo:IAO_0000115>
        <oboInOwl:hasOBONamespace>GAZ</oboInOwl:hasOBONamespace>
        <oboInOwl:id>GAZ:00118528</oboInOwl:id>
        <rdfs:label>Kalaw Township</rdfs:label>
    </owl:NamedIndividual>
    


    <!-- http://purl.obolibrary.org/obo/GAZ_00118529 -->

    <owl:NamedIndividual rdf:about="http://purl.obolibrary.org/obo/GAZ_00118529">
        <obo:RO_0001025 rdf:resource="http://purl.obolibrary.org/obo/GAZ_00025564"/>
        <obo:IAO_0000115>A populated place. A township of Taunggyi District in the Shan State of Myanmar. The principal town is Ywangan.</obo:IAO_0000115>
        <oboInOwl:hasOBONamespace>GAZ</oboInOwl:hasOBONamespace>
        <oboInOwl:id>GAZ:00118529</oboInOwl:id>
        <rdfs:label>Ywangan Township</rdfs:label>
    </owl:NamedIndividual>
    


    <!-- http://purl.obolibrary.org/obo/GAZ_00118530 -->

    <owl:NamedIndividual rdf:about="http://purl.obolibrary.org/obo/GAZ_00118530">
        <obo:RO_0001025 rdf:resource="http://purl.obolibrary.org/obo/GAZ_00025564"/>
        <obo:IAO_0000115>A populated place. A township of Taunggyi District in the Shan State of Myanmar. The principal town is Hopong.</obo:IAO_0000115>
        <oboInOwl:hasOBONamespace>GAZ</oboInOwl:hasOBONamespace>
        <oboInOwl:id>GAZ:00118530</oboInOwl:id>
        <rdfs:label>Hopong Township</rdfs:label>
    </owl:NamedIndividual>
    


    <!-- http://purl.obolibrary.org/obo/GAZ_00118531 -->

    <owl:NamedIndividual rdf:about="http://purl.obolibrary.org/obo/GAZ_00118531">
        <obo:RO_0001025 rdf:resource="http://purl.obolibrary.org/obo/GAZ_00025559"/>
        <obo:IAO_0000115>A populated place. A township of Loilen District in the Shan State of Myanmar. The principal town is Kunhing.</obo:IAO_0000115>
        <oboInOwl:hasOBONamespace>GAZ</oboInOwl:hasOBONamespace>
        <oboInOwl:id>GAZ:00118531</oboInOwl:id>
        <rdfs:label>Kunhing Township</rdfs:label>
    </owl:NamedIndividual>
    


    <!-- http://purl.obolibrary.org/obo/GAZ_00118532 -->

    <owl:NamedIndividual rdf:about="http://purl.obolibrary.org/obo/GAZ_00118532">
        <obo:RO_0001025 rdf:resource="http://purl.obolibrary.org/obo/GAZ_00025559"/>
        <obo:IAO_0000115>A populated place. A township of Loilen District in the Shan State of Myanmar. The principal town is Mawkmai.</obo:IAO_0000115>
        <oboInOwl:hasOBONamespace>GAZ</oboInOwl:hasOBONamespace>
        <oboInOwl:id>GAZ:00118532</oboInOwl:id>
        <rdfs:label>Mawkmai Township</rdfs:label>
    </owl:NamedIndividual>
    


    <!-- http://purl.obolibrary.org/obo/GAZ_00118533 -->

    <owl:NamedIndividual rdf:about="http://purl.obolibrary.org/obo/GAZ_00118533">
        <obo:RO_0001025 rdf:resource="http://purl.obolibrary.org/obo/GAZ_00025559"/>
        <obo:IAO_0000115>A populated place. A township of Loilen District in the Shan State of Myanmar. The principal town is Mong Hsu.</obo:IAO_0000115>
        <oboInOwl:hasOBONamespace>GAZ</oboInOwl:hasOBONamespace>
        <oboInOwl:id>GAZ:00118533</oboInOwl:id>
        <rdfs:label>Mong Hsu Township</rdfs:label>
    </owl:NamedIndividual>
    


    <!-- http://purl.obolibrary.org/obo/GAZ_00118534 -->

    <owl:NamedIndividual rdf:about="http://purl.obolibrary.org/obo/GAZ_00118534">
        <obo:RO_0001025 rdf:resource="http://purl.obolibrary.org/obo/GAZ_00025559"/>
        <obo:IAO_0000115>A populated place. A township of Loilen District in the Shan State of Myanmar. The principal town is Loilen.</obo:IAO_0000115>
        <oboInOwl:hasOBONamespace>GAZ</oboInOwl:hasOBONamespace>
        <oboInOwl:id>GAZ:00118534</oboInOwl:id>
        <rdfs:label>Loilen Township</rdfs:label>
    </owl:NamedIndividual>
    


    <!-- http://purl.obolibrary.org/obo/GAZ_00118535 -->

    <owl:NamedIndividual rdf:about="http://purl.obolibrary.org/obo/GAZ_00118535">
        <obo:RO_0001025 rdf:resource="http://purl.obolibrary.org/obo/GAZ_00025559"/>
        <obo:IAO_0000115>A populated place. A township of Loilen District in the Shan State of Burma. The principal town is Kyethi.</obo:IAO_0000115>
        <oboInOwl:hasOBONamespace>GAZ</oboInOwl:hasOBONamespace>
        <oboInOwl:id>GAZ:00118535</oboInOwl:id>
        <rdfs:label>Kyethi Township</rdfs:label>
    </owl:NamedIndividual>
    


    <!-- http://purl.obolibrary.org/obo/GAZ_00118536 -->

    <owl:NamedIndividual rdf:about="http://purl.obolibrary.org/obo/GAZ_00118536">
        <obo:RO_0001025 rdf:resource="http://purl.obolibrary.org/obo/GAZ_00025559"/>
        <obo:IAO_0000115>A populated place. A township of Loilen District in the Shan State of Myanmar. The principal town is Mong Nai. The Salween River bounds it on the east.</obo:IAO_0000115>
        <oboInOwl:hasOBONamespace>GAZ</oboInOwl:hasOBONamespace>
        <oboInOwl:id>GAZ:00118536</oboInOwl:id>
        <rdfs:label>Mong Nai Township</rdfs:label>
    </owl:NamedIndividual>
    


    <!-- http://purl.obolibrary.org/obo/GAZ_00118537 -->

    <owl:NamedIndividual rdf:about="http://purl.obolibrary.org/obo/GAZ_00118537">
        <obo:RO_0001025 rdf:resource="http://purl.obolibrary.org/obo/GAZ_00025559"/>
        <obo:IAO_0000115>A populated place. A township of Loilen District in the Shan State of Myanmar. The principal town is Mong Pan. To the south it borders Mae Hong Son Province in Thailand and lies west of the Salween River.</obo:IAO_0000115>
        <oboInOwl:hasOBONamespace>GAZ</oboInOwl:hasOBONamespace>
        <oboInOwl:id>GAZ:00118537</oboInOwl:id>
        <rdfs:label>Mong Pan Township</rdfs:label>
    </owl:NamedIndividual>
    


    <!-- http://purl.obolibrary.org/obo/GAZ_00118538 -->

    <owl:NamedIndividual rdf:about="http://purl.obolibrary.org/obo/GAZ_00118538">
        <obo:RO_0001025 rdf:resource="http://purl.obolibrary.org/obo/GAZ_00025559"/>
        <obo:IAO_0000115>A populated place. A township of Loilen District in the Shan State of Myanmar. The principal town is Lai-Hka.</obo:IAO_0000115>
        <oboInOwl:hasOBONamespace>GAZ</oboInOwl:hasOBONamespace>
        <oboInOwl:id>GAZ:00118538</oboInOwl:id>
        <rdfs:label>Lai-Hka Township</rdfs:label>
    </owl:NamedIndividual>
    


    <!-- http://purl.obolibrary.org/obo/GAZ_00118539 -->

    <owl:NamedIndividual rdf:about="http://purl.obolibrary.org/obo/GAZ_00118539">
        <obo:RO_0001025 rdf:resource="http://purl.obolibrary.org/obo/GAZ_00025559"/>
        <obo:IAO_0000115>A populated place. A township of Loilen District in the Shan State of Burma. The principal town is Mong Kung.</obo:IAO_0000115>
        <oboInOwl:hasOBONamespace>GAZ</oboInOwl:hasOBONamespace>
        <oboInOwl:id>GAZ:00118539</oboInOwl:id>
        <rdfs:label>Mong Kung Township</rdfs:label>
    </owl:NamedIndividual>
    


    <!-- http://purl.obolibrary.org/obo/GAZ_00118540 -->

    <owl:NamedIndividual rdf:about="http://purl.obolibrary.org/obo/GAZ_00118540">
        <obo:RO_0001025 rdf:resource="http://purl.obolibrary.org/obo/GAZ_00025559"/>
        <obo:IAO_0000115>A populated place. A township of Loilen District in the Shan State of Burma. The principal town is Langkho.</obo:IAO_0000115>
        <oboInOwl:hasOBONamespace>GAZ</oboInOwl:hasOBONamespace>
        <oboInOwl:id>GAZ:00118540</oboInOwl:id>
        <rdfs:label>Langkho Township</rdfs:label>
    </owl:NamedIndividual>
    


    <!-- http://purl.obolibrary.org/obo/GAZ_00118541 -->

    <owl:NamedIndividual rdf:about="http://purl.obolibrary.org/obo/GAZ_00118541">
        <obo:RO_0001025 rdf:resource="http://purl.obolibrary.org/obo/GAZ_00025559"/>
        <obo:IAO_0000115>A populated place. A township of Loilen District in the Shan State of Myanmar. The principal town is Nansang.</obo:IAO_0000115>
        <oboInOwl:hasOBONamespace>GAZ</oboInOwl:hasOBONamespace>
        <oboInOwl:id>GAZ:00118541</oboInOwl:id>
        <rdfs:label>Nansang Township</rdfs:label>
    </owl:NamedIndividual>
    


    <!-- http://purl.obolibrary.org/obo/GAZ_00118542 -->

    <owl:NamedIndividual rdf:about="http://purl.obolibrary.org/obo/GAZ_00118542">
        <obo:RO_0001025 rdf:resource="http://purl.obolibrary.org/obo/GAZ_00025557"/>
        <obo:IAO_0000115>A populated place. A township of Lashio District in the Shan State of eastern Burma. The principal town is Mongyai.</obo:IAO_0000115>
        <oboInOwl:hasOBONamespace>GAZ</oboInOwl:hasOBONamespace>
        <oboInOwl:id>GAZ:00118542</oboInOwl:id>
        <rdfs:label>Mongyai Township</rdfs:label>
    </owl:NamedIndividual>
    


    <!-- http://purl.obolibrary.org/obo/GAZ_00118543 -->

    <owl:NamedIndividual rdf:about="http://purl.obolibrary.org/obo/GAZ_00118543">
        <obo:RO_0001025 rdf:resource="http://purl.obolibrary.org/obo/GAZ_00025557"/>
        <obo:IAO_0000115>A populated place. A township of Lashio District in the Shan State of eastern Burma. The principal town is Lashio.</obo:IAO_0000115>
        <oboInOwl:hasOBONamespace>GAZ</oboInOwl:hasOBONamespace>
        <oboInOwl:id>GAZ:00118543</oboInOwl:id>
        <rdfs:label>Lashio Township</rdfs:label>
    </owl:NamedIndividual>
    


    <!-- http://purl.obolibrary.org/obo/GAZ_00118544 -->

    <owl:NamedIndividual rdf:about="http://purl.obolibrary.org/obo/GAZ_00118544">
        <obo:RO_0001025 rdf:resource="http://purl.obolibrary.org/obo/GAZ_00025557"/>
        <obo:IAO_0000115>A populated place. A township of Lashio District in the Shan State of eastern Burma. The principal town is Tangyan.</obo:IAO_0000115>
        <oboInOwl:hasOBONamespace>GAZ</oboInOwl:hasOBONamespace>
        <oboInOwl:id>GAZ:00118544</oboInOwl:id>
        <rdfs:label>Tangyan Township</rdfs:label>
    </owl:NamedIndividual>
    


    <!-- http://purl.obolibrary.org/obo/GAZ_00118545 -->

    <owl:NamedIndividual rdf:about="http://purl.obolibrary.org/obo/GAZ_00118545">
        <obo:RO_0001025 rdf:resource="http://purl.obolibrary.org/obo/GAZ_00025557"/>
        <obo:IAO_0000115>A populated place. A township of Lashio District in the Shan State of eastern Burma.</obo:IAO_0000115>
        <oboInOwl:hasOBONamespace>GAZ</oboInOwl:hasOBONamespace>
        <oboInOwl:id>GAZ:00118545</oboInOwl:id>
        <rdfs:label>Hseni Township</rdfs:label>
    </owl:NamedIndividual>
    


    <!-- http://purl.obolibrary.org/obo/GAZ_00118546 -->

    <owl:NamedIndividual rdf:about="http://purl.obolibrary.org/obo/GAZ_00118546">
        <obo:RO_0001025 rdf:resource="http://purl.obolibrary.org/obo/GAZ_00025561"/>
        <obo:IAO_0000115>A populated place. A township of Mong Hsat District in the Shan State of Myanmar. The principal town is Mong Hsat.</obo:IAO_0000115>
        <oboInOwl:hasOBONamespace>GAZ</oboInOwl:hasOBONamespace>
        <oboInOwl:id>GAZ:00118546</oboInOwl:id>
        <rdfs:label>Mong Hsat Township</rdfs:label>
    </owl:NamedIndividual>
    


    <!-- http://purl.obolibrary.org/obo/GAZ_00118547 -->

    <owl:NamedIndividual rdf:about="http://purl.obolibrary.org/obo/GAZ_00118547">
        <obo:RO_0001025 rdf:resource="http://purl.obolibrary.org/obo/GAZ_00025561"/>
        <obo:IAO_0000115>A populated place. A township of Monghsat District in the Shan State of Myanmar. The principal town is Mong Ping.</obo:IAO_0000115>
        <oboInOwl:hasOBONamespace>GAZ</oboInOwl:hasOBONamespace>
        <oboInOwl:id>GAZ:00118547</oboInOwl:id>
        <rdfs:label>Mong Ping Township</rdfs:label>
    </owl:NamedIndividual>
    


    <!-- http://purl.obolibrary.org/obo/GAZ_00118548 -->

    <owl:NamedIndividual rdf:about="http://purl.obolibrary.org/obo/GAZ_00118548">
        <obo:RO_0001025 rdf:resource="http://purl.obolibrary.org/obo/GAZ_00025561"/>
        <obo:IAO_0000115>A populated place. A township of Mongsat District in the Shan State of Myanmar. The principal town is Mong Tong.</obo:IAO_0000115>
        <oboInOwl:hasOBONamespace>GAZ</oboInOwl:hasOBONamespace>
        <oboInOwl:id>GAZ:00118548</oboInOwl:id>
        <rdfs:label>Mong Tong Township</rdfs:label>
    </owl:NamedIndividual>
    


    <!-- http://purl.obolibrary.org/obo/GAZ_00118549 -->

    <owl:NamedIndividual rdf:about="http://purl.obolibrary.org/obo/GAZ_00118549">
        <obo:RO_0001025 rdf:resource="http://purl.obolibrary.org/obo/GAZ_00025563"/>
        <obo:IAO_0000115>A populated place. A township of Tachileik District in the Shan State of Myanmar. The principal town is Tachileik.</obo:IAO_0000115>
        <oboInOwl:hasOBONamespace>GAZ</oboInOwl:hasOBONamespace>
        <oboInOwl:id>GAZ:00118549</oboInOwl:id>
        <rdfs:label>Tachileik Township</rdfs:label>
    </owl:NamedIndividual>
    


    <!-- http://purl.obolibrary.org/obo/GAZ_00118550 -->

    <owl:NamedIndividual rdf:about="http://purl.obolibrary.org/obo/GAZ_00118550">
        <obo:RO_0001025 rdf:resource="http://purl.obolibrary.org/obo/GAZ_00025560"/>
        <obo:IAO_0000115>A populated place. A township of Mong Hpayak District in the Shan State of Myanmar. The principal town is Mong Hpayak.</obo:IAO_0000115>
        <oboInOwl:hasOBONamespace>GAZ</oboInOwl:hasOBONamespace>
        <oboInOwl:id>GAZ:00118550</oboInOwl:id>
        <rdfs:label>Mong Hpayak Township</rdfs:label>
    </owl:NamedIndividual>
    


    <!-- http://purl.obolibrary.org/obo/GAZ_00118551 -->

    <owl:NamedIndividual rdf:about="http://purl.obolibrary.org/obo/GAZ_00118551">
        <obo:RO_0001025 rdf:resource="http://purl.obolibrary.org/obo/GAZ_00025560"/>
        <obo:IAO_0000115>A populated place. A township of Mong Hpayak District in the Shan State of Myanmar. The principal town is Mong Yawng.</obo:IAO_0000115>
        <oboInOwl:hasOBONamespace>GAZ</oboInOwl:hasOBONamespace>
        <oboInOwl:id>GAZ:00118551</oboInOwl:id>
        <rdfs:label>Mong Yawng Township</rdfs:label>
    </owl:NamedIndividual>
    


    <!-- http://purl.obolibrary.org/obo/GAZ_00118552 -->

    <owl:NamedIndividual rdf:about="http://purl.obolibrary.org/obo/GAZ_00118552">
        <obo:RO_0001025 rdf:resource="http://purl.obolibrary.org/obo/GAZ_00025500"/>
        <obo:IAO_0000115>A populated place. A township of Pathein District in the Ayeyawady Division of Myanmar.</obo:IAO_0000115>
        <oboInOwl:hasOBONamespace>GAZ</oboInOwl:hasOBONamespace>
        <oboInOwl:id>GAZ:00118552</oboInOwl:id>
        <rdfs:label>Pathein Township</rdfs:label>
    </owl:NamedIndividual>
    


    <!-- http://purl.obolibrary.org/obo/GAZ_00118553 -->

    <owl:NamedIndividual rdf:about="http://purl.obolibrary.org/obo/GAZ_00118553">
        <obo:RO_0001025 rdf:resource="http://purl.obolibrary.org/obo/GAZ_00025500"/>
        <obo:IAO_0000115>A populated place. A township of Pathein District in the Ayeyarwady Division of Myanmar.</obo:IAO_0000115>
        <oboInOwl:hasOBONamespace>GAZ</oboInOwl:hasOBONamespace>
        <oboInOwl:id>GAZ:00118553</oboInOwl:id>
        <rdfs:label>Ngapudaw Township</rdfs:label>
    </owl:NamedIndividual>
    


    <!-- http://purl.obolibrary.org/obo/GAZ_00118554 -->

    <owl:NamedIndividual rdf:about="http://purl.obolibrary.org/obo/GAZ_00118554">
        <obo:RO_0001025 rdf:resource="http://purl.obolibrary.org/obo/GAZ_00025500"/>
        <obo:IAO_0000115>A populated place. A township of Pathein District in the Ayeyarwady Division of Myanmar.</obo:IAO_0000115>
        <oboInOwl:hasOBONamespace>GAZ</oboInOwl:hasOBONamespace>
        <oboInOwl:id>GAZ:00118554</oboInOwl:id>
        <rdfs:label>Kangyidaunk Township</rdfs:label>
    </owl:NamedIndividual>
    


    <!-- http://purl.obolibrary.org/obo/GAZ_00118555 -->

    <owl:NamedIndividual rdf:about="http://purl.obolibrary.org/obo/GAZ_00118555">
        <obo:RO_0001025 rdf:resource="http://purl.obolibrary.org/obo/GAZ_00025500"/>
        <obo:IAO_0000115>A populated place. A township of Pathein District in the Ayeyarwady Division of Myanmar. The capital is Kyonpyaw town.</obo:IAO_0000115>
        <oboInOwl:hasOBONamespace>GAZ</oboInOwl:hasOBONamespace>
        <oboInOwl:id>GAZ:00118555</oboInOwl:id>
        <rdfs:label>Kyonpyaw Township</rdfs:label>
    </owl:NamedIndividual>
    


    <!-- http://purl.obolibrary.org/obo/GAZ_00118556 -->

    <owl:NamedIndividual rdf:about="http://purl.obolibrary.org/obo/GAZ_00118556">
        <obo:RO_0001025 rdf:resource="http://purl.obolibrary.org/obo/GAZ_00025500"/>
        <obo:IAO_0000115>A populated place. A township of Pathein District in the Ayeyarwady Division of Myanmar.</obo:IAO_0000115>
        <oboInOwl:hasOBONamespace>GAZ</oboInOwl:hasOBONamespace>
        <oboInOwl:id>GAZ:00118556</oboInOwl:id>
        <rdfs:label>Thabaung Township</rdfs:label>
    </owl:NamedIndividual>
    


    <!-- http://purl.obolibrary.org/obo/GAZ_00118558 -->

    <owl:NamedIndividual rdf:about="http://purl.obolibrary.org/obo/GAZ_00118558">
        <obo:RO_0001025 rdf:resource="http://purl.obolibrary.org/obo/GAZ_00025500"/>
        <obo:IAO_0000115>A populated place. A township of Pathein District in the Ayeyarwady Division of Myanmar.</obo:IAO_0000115>
        <oboInOwl:hasOBONamespace>GAZ</oboInOwl:hasOBONamespace>
        <oboInOwl:id>GAZ:00118558</oboInOwl:id>
        <rdfs:label>Kyaunggon Township</rdfs:label>
    </owl:NamedIndividual>
    


    <!-- http://purl.obolibrary.org/obo/GAZ_00118559 -->

    <owl:NamedIndividual rdf:about="http://purl.obolibrary.org/obo/GAZ_00118559">
        <obo:RO_0001025 rdf:resource="http://purl.obolibrary.org/obo/GAZ_00025500"/>
        <obo:IAO_0000115>A populated place. A township of Pathein District in the Ayeyarwady Division of Myanmar.</obo:IAO_0000115>
        <oboInOwl:hasOBONamespace>GAZ</oboInOwl:hasOBONamespace>
        <oboInOwl:id>GAZ:00118559</oboInOwl:id>
        <rdfs:label>Yekyi Township</rdfs:label>
    </owl:NamedIndividual>
    


    <!-- http://purl.obolibrary.org/obo/GAZ_00118560 -->

    <owl:NamedIndividual rdf:about="http://purl.obolibrary.org/obo/GAZ_00118560">
        <obo:RO_0001025 rdf:resource="http://purl.obolibrary.org/obo/GAZ_00025503"/>
        <obo:IAO_0000115>A populated place. A township of Hinthada District in the Ayeyarwady Division of Myanmar.</obo:IAO_0000115>
        <oboInOwl:hasOBONamespace>GAZ</oboInOwl:hasOBONamespace>
        <oboInOwl:id>GAZ:00118560</oboInOwl:id>
        <rdfs:label>Hinthada Township</rdfs:label>
    </owl:NamedIndividual>
    


    <!-- http://purl.obolibrary.org/obo/GAZ_00118561 -->

    <owl:NamedIndividual rdf:about="http://purl.obolibrary.org/obo/GAZ_00118561">
        <obo:RO_0001025 rdf:resource="http://purl.obolibrary.org/obo/GAZ_00025503"/>
        <obo:IAO_0000115>A populated place. A township of Hinthada District in the Ayeyarwady Division of Myanmar.</obo:IAO_0000115>
        <oboInOwl:hasOBONamespace>GAZ</oboInOwl:hasOBONamespace>
        <oboInOwl:id>GAZ:00118561</oboInOwl:id>
        <rdfs:label>Laymyethna Township</rdfs:label>
    </owl:NamedIndividual>
    


    <!-- http://purl.obolibrary.org/obo/GAZ_00118562 -->

    <owl:NamedIndividual rdf:about="http://purl.obolibrary.org/obo/GAZ_00118562">
        <obo:RO_0001025 rdf:resource="http://purl.obolibrary.org/obo/GAZ_00025503"/>
        <obo:IAO_0000115>A populated place. A township of Hinthada District in the Ayeyarwady Division of Myanmar.</obo:IAO_0000115>
        <oboInOwl:hasOBONamespace>GAZ</oboInOwl:hasOBONamespace>
        <oboInOwl:id>GAZ:00118562</oboInOwl:id>
        <rdfs:label>Ingapu Township</rdfs:label>
    </owl:NamedIndividual>
    


    <!-- http://purl.obolibrary.org/obo/GAZ_00118563 -->

    <owl:NamedIndividual rdf:about="http://purl.obolibrary.org/obo/GAZ_00118563">
        <obo:RO_0001025 rdf:resource="http://purl.obolibrary.org/obo/GAZ_00025503"/>
        <obo:IAO_0000115>A populated place. A township of Hinthada District in the Ayeyarwady Division of Myanmar.</obo:IAO_0000115>
        <oboInOwl:hasOBONamespace>GAZ</oboInOwl:hasOBONamespace>
        <oboInOwl:id>GAZ:00118563</oboInOwl:id>
        <rdfs:label>Zalun Township</rdfs:label>
    </owl:NamedIndividual>
    


    <!-- http://purl.obolibrary.org/obo/GAZ_00118564 -->

    <owl:NamedIndividual rdf:about="http://purl.obolibrary.org/obo/GAZ_00118564">
        <obo:RO_0001025 rdf:resource="http://purl.obolibrary.org/obo/GAZ_00025503"/>
        <obo:IAO_0000115>A populated place. A township of Hinthada District in the Ayeyarwady Division of Myanmar.</obo:IAO_0000115>
        <oboInOwl:hasOBONamespace>GAZ</oboInOwl:hasOBONamespace>
        <oboInOwl:id>GAZ:00118564</oboInOwl:id>
        <rdfs:label>Myanaung Township</rdfs:label>
    </owl:NamedIndividual>
    


    <!-- http://purl.obolibrary.org/obo/GAZ_00118565 -->

    <owl:NamedIndividual rdf:about="http://purl.obolibrary.org/obo/GAZ_00118565">
        <obo:RO_0001025 rdf:resource="http://purl.obolibrary.org/obo/GAZ_00025503"/>
        <obo:IAO_0000115>A populated place. A township of Hinthada District in the Ayeyarwady Division of Myanmar.</obo:IAO_0000115>
        <oboInOwl:hasOBONamespace>GAZ</oboInOwl:hasOBONamespace>
        <oboInOwl:id>GAZ:00118565</oboInOwl:id>
        <rdfs:label>Kyangin Township</rdfs:label>
    </owl:NamedIndividual>
    


    <!-- http://purl.obolibrary.org/obo/GAZ_00118566 -->

    <owl:NamedIndividual rdf:about="http://purl.obolibrary.org/obo/GAZ_00118566">
        <obo:RO_0001025 rdf:resource="http://purl.obolibrary.org/obo/GAZ_00025499"/>
        <obo:IAO_0000115>A populated place. A township of Myaungmya District in the Ayeyarwady Division of Myanmar. The seat is Myaungmya.</obo:IAO_0000115>
        <oboInOwl:hasOBONamespace>GAZ</oboInOwl:hasOBONamespace>
        <oboInOwl:id>GAZ:00118566</oboInOwl:id>
        <rdfs:label>Myaungmya Township</rdfs:label>
    </owl:NamedIndividual>
    


    <!-- http://purl.obolibrary.org/obo/GAZ_00118567 -->

    <owl:NamedIndividual rdf:about="http://purl.obolibrary.org/obo/GAZ_00118567">
        <obo:RO_0001025 rdf:resource="http://purl.obolibrary.org/obo/GAZ_00025499"/>
        <obo:IAO_0000115>A populated place. A township of Myaungmya District in the Ayeyarwady Division of Myanmar.</obo:IAO_0000115>
        <oboInOwl:hasOBONamespace>GAZ</oboInOwl:hasOBONamespace>
        <oboInOwl:id>GAZ:00118567</oboInOwl:id>
        <rdfs:label>Labutta Township</rdfs:label>
    </owl:NamedIndividual>
    


    <!-- http://purl.obolibrary.org/obo/GAZ_00118568 -->

    <owl:NamedIndividual rdf:about="http://purl.obolibrary.org/obo/GAZ_00118568">
        <obo:RO_0001025 rdf:resource="http://purl.obolibrary.org/obo/GAZ_00025499"/>
        <obo:IAO_0000115>A populated place. A township of Myaungmya District in the Ayeyarwady Division of Myanmar.</obo:IAO_0000115>
        <oboInOwl:hasOBONamespace>GAZ</oboInOwl:hasOBONamespace>
        <oboInOwl:id>GAZ:00118568</oboInOwl:id>
        <rdfs:label>Mawlamyinegyun Township</rdfs:label>
    </owl:NamedIndividual>
    


    <!-- http://purl.obolibrary.org/obo/GAZ_00118569 -->

    <owl:NamedIndividual rdf:about="http://purl.obolibrary.org/obo/GAZ_00118569">
        <obo:RO_0001025 rdf:resource="http://purl.obolibrary.org/obo/GAZ_00025499"/>
        <obo:IAO_0000115>A populated place. A township of Myaungmya District in the Ayeyarwady Division of Myanmar. The townsjhip is connected to the Einme Township across the Kyungon Bridge on the Pyanmalot River.</obo:IAO_0000115>
        <oboInOwl:hasOBONamespace>GAZ</oboInOwl:hasOBONamespace>
        <oboInOwl:id>GAZ:00118569</oboInOwl:id>
        <rdfs:label>Wakema Township</rdfs:label>
    </owl:NamedIndividual>
    


    <!-- http://purl.obolibrary.org/obo/GAZ_00118570 -->

    <owl:NamedIndividual rdf:about="http://purl.obolibrary.org/obo/GAZ_00118570">
        <obo:RO_0001025 rdf:resource="http://purl.obolibrary.org/obo/GAZ_00025499"/>
        <obo:IAO_0000115>A populated place. A township of Myaungmya District in the Ayeyarwady Division of Myanmar.</obo:IAO_0000115>
        <oboInOwl:hasOBONamespace>GAZ</oboInOwl:hasOBONamespace>
        <oboInOwl:id>GAZ:00118570</oboInOwl:id>
        <rdfs:label>Einme Township</rdfs:label>
    </owl:NamedIndividual>
    


    <!-- http://purl.obolibrary.org/obo/GAZ_00118571 -->

    <owl:NamedIndividual rdf:about="http://purl.obolibrary.org/obo/GAZ_00118571">
        <obo:RO_0001025 rdf:resource="http://purl.obolibrary.org/obo/GAZ_00025502"/>
        <obo:IAO_0000115>A populated place. A township of Ma-Ubin District in the Ayeyarwady Division of Myanmar.</obo:IAO_0000115>
        <oboInOwl:hasOBONamespace>GAZ</oboInOwl:hasOBONamespace>
        <oboInOwl:id>GAZ:00118571</oboInOwl:id>
        <rdfs:label>Nyaungdon Township</rdfs:label>
    </owl:NamedIndividual>
    


    <!-- http://purl.obolibrary.org/obo/GAZ_00118572 -->

    <owl:NamedIndividual rdf:about="http://purl.obolibrary.org/obo/GAZ_00118572">
        <obo:RO_0001025 rdf:resource="http://purl.obolibrary.org/obo/GAZ_00025502"/>
        <obo:IAO_0000115>A populated place. A township of Ma-Ubin District in the Ayeyarwady Division of Myanmar.</obo:IAO_0000115>
        <oboInOwl:hasOBONamespace>GAZ</oboInOwl:hasOBONamespace>
        <oboInOwl:id>GAZ:00118572</oboInOwl:id>
        <rdfs:label>Maubin Township</rdfs:label>
    </owl:NamedIndividual>
    


    <!-- http://purl.obolibrary.org/obo/GAZ_00118573 -->

    <owl:NamedIndividual rdf:about="http://purl.obolibrary.org/obo/GAZ_00118573">
        <obo:RO_0001025 rdf:resource="http://purl.obolibrary.org/obo/GAZ_00025502"/>
        <obo:IAO_0000115>A populated place. A township of Ma-Ubin District in the Ayeyarwady Division of Myanmar.</obo:IAO_0000115>
        <oboInOwl:hasOBONamespace>GAZ</oboInOwl:hasOBONamespace>
        <oboInOwl:id>GAZ:00118573</oboInOwl:id>
        <rdfs:label>Danubyu Township</rdfs:label>
    </owl:NamedIndividual>
    


    <!-- http://purl.obolibrary.org/obo/GAZ_00118574 -->

    <owl:NamedIndividual rdf:about="http://purl.obolibrary.org/obo/GAZ_00118574">
        <obo:RO_0001025 rdf:resource="http://purl.obolibrary.org/obo/GAZ_00025502"/>
        <obo:IAO_0000115>A populated place. A township of Ma-Ubin District in the Ayeyarwady Division of Myanmar.</obo:IAO_0000115>
        <oboInOwl:hasOBONamespace>GAZ</oboInOwl:hasOBONamespace>
        <oboInOwl:id>GAZ:00118574</oboInOwl:id>
        <rdfs:label>Pantanaw Township</rdfs:label>
    </owl:NamedIndividual>
    


    <!-- http://purl.obolibrary.org/obo/GAZ_00118575 -->

    <owl:NamedIndividual rdf:about="http://purl.obolibrary.org/obo/GAZ_00118575">
        <obo:RO_0001025 rdf:resource="http://purl.obolibrary.org/obo/GAZ_00025501"/>
        <obo:IAO_0000115>A populated place. A township of Pyapon District in the Ayeyarwady Division of Myanmar.</obo:IAO_0000115>
        <oboInOwl:hasOBONamespace>GAZ</oboInOwl:hasOBONamespace>
        <oboInOwl:id>GAZ:00118575</oboInOwl:id>
        <rdfs:label>Kyaiklat Township</rdfs:label>
    </owl:NamedIndividual>
    


    <!-- http://purl.obolibrary.org/obo/GAZ_00118576 -->

    <owl:NamedIndividual rdf:about="http://purl.obolibrary.org/obo/GAZ_00118576">
        <obo:RO_0001025 rdf:resource="http://purl.obolibrary.org/obo/GAZ_00025501"/>
        <obo:IAO_0000115>A populated place. A township of Pyapon District in the Ayeyarwady Division of Myanmar.</obo:IAO_0000115>
        <oboInOwl:hasOBONamespace>GAZ</oboInOwl:hasOBONamespace>
        <oboInOwl:id>GAZ:00118576</oboInOwl:id>
        <rdfs:label>Bogale Township</rdfs:label>
    </owl:NamedIndividual>
    


    <!-- http://purl.obolibrary.org/obo/GAZ_00118577 -->

    <owl:NamedIndividual rdf:about="http://purl.obolibrary.org/obo/GAZ_00118577">
        <obo:RO_0001025 rdf:resource="http://purl.obolibrary.org/obo/GAZ_00025501"/>
        <obo:IAO_0000115>A populated place. A township of Pyapon District in the Ayeyarwady Division of Myanmar.</obo:IAO_0000115>
        <oboInOwl:hasOBONamespace>GAZ</oboInOwl:hasOBONamespace>
        <oboInOwl:id>GAZ:00118577</oboInOwl:id>
        <rdfs:label>Dedaye Township</rdfs:label>
    </owl:NamedIndividual>
    


    <!-- http://purl.obolibrary.org/obo/GAZ_00118578 -->

    <owl:NamedIndividual rdf:about="http://purl.obolibrary.org/obo/GAZ_00118578">
        <obo:RO_0001025 rdf:resource="http://purl.obolibrary.org/obo/GAZ_00025501"/>
        <obo:IAO_0000115>A populated place. A township of Pyapon District in the Ayeyarwady Division of Myanmar.</obo:IAO_0000115>
        <oboInOwl:hasOBONamespace>GAZ</oboInOwl:hasOBONamespace>
        <oboInOwl:id>GAZ:00118578</oboInOwl:id>
        <rdfs:label>Pyapon Township</rdfs:label>
    </owl:NamedIndividual>
    


    <!-- http://purl.obolibrary.org/obo/GAZ_00118579 -->

    <owl:NamedIndividual rdf:about="http://purl.obolibrary.org/obo/GAZ_00118579">
        <obo:RO_0001025 rdf:resource="http://purl.obolibrary.org/obo/GAZ_00025511"/>
        <obo:IAO_0000115>A populated place. A township of Magway District in the Magway Division of Myanmar. The principal town is Yenangyaung.</obo:IAO_0000115>
        <oboInOwl:hasOBONamespace>GAZ</oboInOwl:hasOBONamespace>
        <oboInOwl:id>GAZ:00118579</oboInOwl:id>
        <rdfs:label>Yenangyaung Township</rdfs:label>
    </owl:NamedIndividual>
    


    <!-- http://purl.obolibrary.org/obo/GAZ_00118580 -->

    <owl:NamedIndividual rdf:about="http://purl.obolibrary.org/obo/GAZ_00118580">
        <obo:RO_0001025 rdf:resource="http://purl.obolibrary.org/obo/GAZ_00025511"/>
        <obo:IAO_0000115>A populated place. A township of Magway District in the Magway Division of Myanmar. The principal town is Chauck.</obo:IAO_0000115>
        <oboInOwl:hasOBONamespace>GAZ</oboInOwl:hasOBONamespace>
        <oboInOwl:id>GAZ:00118580</oboInOwl:id>
        <rdfs:label>Chauck Township</rdfs:label>
    </owl:NamedIndividual>
    


    <!-- http://purl.obolibrary.org/obo/GAZ_00118581 -->

    <owl:NamedIndividual rdf:about="http://purl.obolibrary.org/obo/GAZ_00118581">
        <obo:RO_0001025 rdf:resource="http://purl.obolibrary.org/obo/GAZ_00025511"/>
        <obo:IAO_0000115>A populated place. A township of Magway District in the Magway Division of Myanmar. The principal town is Natmauk.</obo:IAO_0000115>
        <oboInOwl:hasOBONamespace>GAZ</oboInOwl:hasOBONamespace>
        <oboInOwl:id>GAZ:00118581</oboInOwl:id>
        <rdfs:label>Natmauk Township</rdfs:label>
    </owl:NamedIndividual>
    


    <!-- http://purl.obolibrary.org/obo/GAZ_00118582 -->

    <owl:NamedIndividual rdf:about="http://purl.obolibrary.org/obo/GAZ_00118582">
        <obo:RO_0001025 rdf:resource="http://purl.obolibrary.org/obo/GAZ_00025511"/>
        <obo:IAO_0000115>A populated place. A township of Magway District in the Magway Division of Myanmar. The principal town is Magway.</obo:IAO_0000115>
        <oboInOwl:hasOBONamespace>GAZ</oboInOwl:hasOBONamespace>
        <oboInOwl:id>GAZ:00118582</oboInOwl:id>
        <rdfs:label>Magway Township</rdfs:label>
    </owl:NamedIndividual>
    


    <!-- http://purl.obolibrary.org/obo/GAZ_00118583 -->

    <owl:NamedIndividual rdf:about="http://purl.obolibrary.org/obo/GAZ_00118583">
        <obo:RO_0001025 rdf:resource="http://purl.obolibrary.org/obo/GAZ_00025511"/>
        <obo:IAO_0000115>A populated place. A township of Magway District in the Magway Division of Myanmar. The principal town is Myothit.</obo:IAO_0000115>
        <oboInOwl:hasOBONamespace>GAZ</oboInOwl:hasOBONamespace>
        <oboInOwl:id>GAZ:00118583</oboInOwl:id>
        <rdfs:label>Myothit Township</rdfs:label>
    </owl:NamedIndividual>
    


    <!-- http://purl.obolibrary.org/obo/GAZ_00118584 -->

    <owl:NamedIndividual rdf:about="http://purl.obolibrary.org/obo/GAZ_00118584">
        <obo:RO_0001025 rdf:resource="http://purl.obolibrary.org/obo/GAZ_00025511"/>
        <obo:IAO_0000115>A populated place. A township of Magway District in the Magway Division of Myanmar. The principal town is Taungdwingyi.</obo:IAO_0000115>
        <oboInOwl:hasOBONamespace>GAZ</oboInOwl:hasOBONamespace>
        <oboInOwl:id>GAZ:00118584</oboInOwl:id>
        <rdfs:label>Taungdwingyi Township</rdfs:label>
    </owl:NamedIndividual>
    


    <!-- http://purl.obolibrary.org/obo/GAZ_00118585 -->

    <owl:NamedIndividual rdf:about="http://purl.obolibrary.org/obo/GAZ_00118585">
        <obo:RO_0001025 rdf:resource="http://purl.obolibrary.org/obo/GAZ_00025509"/>
        <obo:IAO_0000115>A populated place. A township of Gangaw District in the Magway Division of Myanmar. The principal town is Tilin.</obo:IAO_0000115>
        <oboInOwl:hasOBONamespace>GAZ</oboInOwl:hasOBONamespace>
        <oboInOwl:id>GAZ:00118585</oboInOwl:id>
        <rdfs:label>Tilin Township</rdfs:label>
    </owl:NamedIndividual>
    


    <!-- http://purl.obolibrary.org/obo/GAZ_00118586 -->

    <owl:NamedIndividual rdf:about="http://purl.obolibrary.org/obo/GAZ_00118586">
        <obo:RO_0001025 rdf:resource="http://purl.obolibrary.org/obo/GAZ_00025509"/>
        <obo:IAO_0000115>A populated place. A township of Gangaw District in the Magway Division of Myanmar. The principal town is Saw.</obo:IAO_0000115>
        <oboInOwl:hasOBONamespace>GAZ</oboInOwl:hasOBONamespace>
        <oboInOwl:id>GAZ:00118586</oboInOwl:id>
        <rdfs:label>Saw Township</rdfs:label>
    </owl:NamedIndividual>
    


    <!-- http://purl.obolibrary.org/obo/GAZ_00118587 -->

    <owl:NamedIndividual rdf:about="http://purl.obolibrary.org/obo/GAZ_00118587">
        <obo:RO_0001025 rdf:resource="http://purl.obolibrary.org/obo/GAZ_00025509"/>
        <obo:IAO_0000115>A populated place. A township of Gangaw District in the Magway Division of Myanmar. The principal town is Gangaw.</obo:IAO_0000115>
        <oboInOwl:hasOBONamespace>GAZ</oboInOwl:hasOBONamespace>
        <oboInOwl:id>GAZ:00118587</oboInOwl:id>
        <rdfs:label>Gangaw Township</rdfs:label>
    </owl:NamedIndividual>
    


    <!-- http://purl.obolibrary.org/obo/GAZ_00118588 -->

    <owl:NamedIndividual rdf:about="http://purl.obolibrary.org/obo/GAZ_00118588">
        <obo:RO_0001025 rdf:resource="http://purl.obolibrary.org/obo/GAZ_00025512"/>
        <obo:IAO_0000115>A populated place. A township of Minbu District in the Magway Division of Myanmar. The principal town is Minbu.</obo:IAO_0000115>
        <oboInOwl:hasOBONamespace>GAZ</oboInOwl:hasOBONamespace>
        <oboInOwl:id>GAZ:00118588</oboInOwl:id>
        <rdfs:label>Minbu Township</rdfs:label>
    </owl:NamedIndividual>
    


    <!-- http://purl.obolibrary.org/obo/GAZ_00118589 -->

    <owl:NamedIndividual rdf:about="http://purl.obolibrary.org/obo/GAZ_00118589">
        <obo:RO_0001025 rdf:resource="http://purl.obolibrary.org/obo/GAZ_00025512"/>
        <obo:IAO_0000115>A populated place. A township of Minbu District in the Magway Division of Myanmar. The principal town is Ngape.</obo:IAO_0000115>
        <oboInOwl:hasOBONamespace>GAZ</oboInOwl:hasOBONamespace>
        <oboInOwl:id>GAZ:00118589</oboInOwl:id>
        <rdfs:label>Ngape Township</rdfs:label>
    </owl:NamedIndividual>
    


    <!-- http://purl.obolibrary.org/obo/GAZ_00118590 -->

    <owl:NamedIndividual rdf:about="http://purl.obolibrary.org/obo/GAZ_00118590">
        <obo:RO_0001025 rdf:resource="http://purl.obolibrary.org/obo/GAZ_00025512"/>
        <obo:IAO_0000115>A populated place. A township of Minbu District in the Magway Division of Myanmar. The principal town is Sidoktaya.</obo:IAO_0000115>
        <oboInOwl:hasOBONamespace>GAZ</oboInOwl:hasOBONamespace>
        <oboInOwl:id>GAZ:00118590</oboInOwl:id>
        <rdfs:label>Sidoktaya Township</rdfs:label>
    </owl:NamedIndividual>
    


    <!-- http://purl.obolibrary.org/obo/GAZ_00118591 -->

    <owl:NamedIndividual rdf:about="http://purl.obolibrary.org/obo/GAZ_00118591">
        <obo:RO_0001025 rdf:resource="http://purl.obolibrary.org/obo/GAZ_00025512"/>
        <obo:IAO_0000115>A populated place. A township of Minbu District in the Magway Division of Myanmar. The principal town is Salin.</obo:IAO_0000115>
        <oboInOwl:hasOBONamespace>GAZ</oboInOwl:hasOBONamespace>
        <oboInOwl:id>GAZ:00118591</oboInOwl:id>
        <rdfs:label>Salin Township</rdfs:label>
    </owl:NamedIndividual>
    


    <!-- http://purl.obolibrary.org/obo/GAZ_00118592 -->

    <owl:NamedIndividual rdf:about="http://purl.obolibrary.org/obo/GAZ_00118592">
        <obo:RO_0001025 rdf:resource="http://purl.obolibrary.org/obo/GAZ_00025512"/>
        <obo:IAO_0000115>A populated place. A township of Minbu District in the Magway Division of Myanmar. The principal town is Pwintbyu.</obo:IAO_0000115>
        <oboInOwl:hasOBONamespace>GAZ</oboInOwl:hasOBONamespace>
        <oboInOwl:id>GAZ:00118592</oboInOwl:id>
        <rdfs:label>Pwintbyu Township</rdfs:label>
    </owl:NamedIndividual>
    


    <!-- http://purl.obolibrary.org/obo/GAZ_00118593 -->

    <owl:NamedIndividual rdf:about="http://purl.obolibrary.org/obo/GAZ_00118593">
        <rdf:type rdf:resource="http://purl.obolibrary.org/obo/ENVO_00000004"/>
        <obo:RO_0001025 rdf:resource="http://purl.obolibrary.org/obo/GAZ_02000000"/>
        <obo:IAO_0000115>A district of the Taninthayi Division of Myanmar.</obo:IAO_0000115>
        <oboInOwl:hasOBONamespace>GAZ</oboInOwl:hasOBONamespace>
        <oboInOwl:id>GAZ:00118593</oboInOwl:id>
        <rdfs:label>Kawthoung District</rdfs:label>
    </owl:NamedIndividual>
    


    <!-- http://purl.obolibrary.org/obo/GAZ_00118594 -->

    <owl:NamedIndividual rdf:about="http://purl.obolibrary.org/obo/GAZ_00118594">
        <rdf:type rdf:resource="http://purl.obolibrary.org/obo/ENVO_00000004"/>
        <obo:RO_0001025 rdf:resource="http://purl.obolibrary.org/obo/GAZ_02000000"/>
        <obo:IAO_0000115>A district of the Taninthayi Division of Myanmar.</obo:IAO_0000115>
        <oboInOwl:hasOBONamespace>GAZ</oboInOwl:hasOBONamespace>
        <oboInOwl:id>GAZ:00118594</oboInOwl:id>
        <rdfs:label>Dawei District</rdfs:label>
    </owl:NamedIndividual>
    


    <!-- http://purl.obolibrary.org/obo/GAZ_00118595 -->

    <owl:NamedIndividual rdf:about="http://purl.obolibrary.org/obo/GAZ_00118595">
        <rdf:type rdf:resource="http://purl.obolibrary.org/obo/ENVO_00000004"/>
        <obo:RO_0001025 rdf:resource="http://purl.obolibrary.org/obo/GAZ_02000000"/>
        <obo:IAO_0000115>A district of the Taninthayi Division of Myanmar.</obo:IAO_0000115>
        <oboInOwl:hasOBONamespace>GAZ</oboInOwl:hasOBONamespace>
        <oboInOwl:id>GAZ:00118595</oboInOwl:id>
        <rdfs:label>Myeik District</rdfs:label>
    </owl:NamedIndividual>
    


    <!-- http://purl.obolibrary.org/obo/GAZ_00118596 -->

    <owl:NamedIndividual rdf:about="http://purl.obolibrary.org/obo/GAZ_00118596">
        <obo:RO_0001025 rdf:resource="http://purl.obolibrary.org/obo/GAZ_00118594"/>
        <oboInOwl:hasOBONamespace>GAZ</oboInOwl:hasOBONamespace>
        <oboInOwl:id>GAZ:00118596</oboInOwl:id>
        <rdfs:label>Thayetchaung Township</rdfs:label>
    </owl:NamedIndividual>
    


    <!-- http://purl.obolibrary.org/obo/GAZ_00118597 -->

    <owl:NamedIndividual rdf:about="http://purl.obolibrary.org/obo/GAZ_00118597">
        <obo:RO_0001025 rdf:resource="http://purl.obolibrary.org/obo/GAZ_00118594"/>
        <obo:IAO_0000115>A populated place. A township of Dawei District in the Taninthayi Division of Myanmar.</obo:IAO_0000115>
        <oboInOwl:hasOBONamespace>GAZ</oboInOwl:hasOBONamespace>
        <oboInOwl:id>GAZ:00118597</oboInOwl:id>
        <rdfs:label>Longlon Township</rdfs:label>
    </owl:NamedIndividual>
    


    <!-- http://purl.obolibrary.org/obo/GAZ_00118598 -->

    <owl:NamedIndividual rdf:about="http://purl.obolibrary.org/obo/GAZ_00118598">
        <obo:RO_0001025 rdf:resource="http://purl.obolibrary.org/obo/GAZ_00118594"/>
        <oboInOwl:hasOBONamespace>GAZ</oboInOwl:hasOBONamespace>
        <oboInOwl:id>GAZ:00118598</oboInOwl:id>
        <rdfs:label>Yebyu Township</rdfs:label>
    </owl:NamedIndividual>
    


    <!-- http://purl.obolibrary.org/obo/GAZ_00118599 -->

    <owl:NamedIndividual rdf:about="http://purl.obolibrary.org/obo/GAZ_00118599">
        <obo:RO_0001025 rdf:resource="http://purl.obolibrary.org/obo/GAZ_00118594"/>
        <obo:IAO_0000115>Dawei Township is a township of Dawei District in the Taninthayi Division of Myanmar. The principal town is Dawei.</obo:IAO_0000115>
        <oboInOwl:hasOBONamespace>GAZ</oboInOwl:hasOBONamespace>
        <oboInOwl:id>GAZ:00118599</oboInOwl:id>
        <rdfs:label>Dawei Township</rdfs:label>
    </owl:NamedIndividual>
    


    <!-- http://purl.obolibrary.org/obo/GAZ_00118600 -->

    <owl:NamedIndividual rdf:about="http://purl.obolibrary.org/obo/GAZ_00118600">
        <obo:RO_0001025 rdf:resource="http://purl.obolibrary.org/obo/GAZ_00118593"/>
        <obo:IAO_0000115>A populated place. A township of Kawthoung District in the Taninthayi Division of Myanmar. The principal town is Kawthoung.</obo:IAO_0000115>
        <oboInOwl:hasOBONamespace>GAZ</oboInOwl:hasOBONamespace>
        <oboInOwl:id>GAZ:00118600</oboInOwl:id>
        <rdfs:label>Kawthoung Township</rdfs:label>
    </owl:NamedIndividual>
    


    <!-- http://purl.obolibrary.org/obo/GAZ_00118601 -->

    <owl:NamedIndividual rdf:about="http://purl.obolibrary.org/obo/GAZ_00118601">
        <obo:RO_0001025 rdf:resource="http://purl.obolibrary.org/obo/GAZ_00118593"/>
        <obo:IAO_0000115>A populated place. A township of Kawthoung District in the Taninthayi Division of Myanmar. The principal town is Bokpyin.</obo:IAO_0000115>
        <oboInOwl:hasOBONamespace>GAZ</oboInOwl:hasOBONamespace>
        <oboInOwl:id>GAZ:00118601</oboInOwl:id>
        <rdfs:label>Bokpyin Township</rdfs:label>
    </owl:NamedIndividual>
    


    <!-- http://purl.obolibrary.org/obo/GAZ_00118602 -->

    <owl:NamedIndividual rdf:about="http://purl.obolibrary.org/obo/GAZ_00118602">
        <obo:RO_0001025 rdf:resource="http://purl.obolibrary.org/obo/GAZ_00118595"/>
        <obo:IAO_0000115>A populated place. A township of Myeik District in the Taninthayi Division of Myanmar. The principal town is Myeik.</obo:IAO_0000115>
        <oboInOwl:hasOBONamespace>GAZ</oboInOwl:hasOBONamespace>
        <oboInOwl:id>GAZ:00118602</oboInOwl:id>
        <rdfs:label>Myeik Township</rdfs:label>
    </owl:NamedIndividual>
    


    <!-- http://purl.obolibrary.org/obo/GAZ_00118603 -->

    <owl:NamedIndividual rdf:about="http://purl.obolibrary.org/obo/GAZ_00118603">
        <obo:RO_0001025 rdf:resource="http://purl.obolibrary.org/obo/GAZ_00118595"/>
        <obo:IAO_0000115>A populated place. A township of Myeik District in the Taninthayi Division of Myanmar. The principal town is Kiyttsu.</obo:IAO_0000115>
        <oboInOwl:hasOBONamespace>GAZ</oboInOwl:hasOBONamespace>
        <oboInOwl:id>GAZ:00118603</oboInOwl:id>
        <rdfs:label>Kiyttsu Township</rdfs:label>
    </owl:NamedIndividual>
    


    <!-- http://purl.obolibrary.org/obo/GAZ_00118604 -->

    <owl:NamedIndividual rdf:about="http://purl.obolibrary.org/obo/GAZ_00118604">
        <obo:RO_0001025 rdf:resource="http://purl.obolibrary.org/obo/GAZ_00118595"/>
        <obo:IAO_0000115>A populated place. A township of Myeik District in the Taninthayi Division of Myanmar. The principal town is Taninthayi.</obo:IAO_0000115>
        <oboInOwl:hasOBONamespace>GAZ</oboInOwl:hasOBONamespace>
        <oboInOwl:id>GAZ:00118604</oboInOwl:id>
        <rdfs:label>Taninthayi Township</rdfs:label>
    </owl:NamedIndividual>
    


    <!-- http://purl.obolibrary.org/obo/GAZ_00118605 -->

    <owl:NamedIndividual rdf:about="http://purl.obolibrary.org/obo/GAZ_00118605">
        <obo:RO_0001025 rdf:resource="http://purl.obolibrary.org/obo/GAZ_00118595"/>
        <obo:IAO_0000115>A populated place. A township of Myeik District in the Taninthayi Division of Myanmar. The principal town is Palaw.</obo:IAO_0000115>
        <oboInOwl:hasOBONamespace>GAZ</oboInOwl:hasOBONamespace>
        <oboInOwl:id>GAZ:00118605</oboInOwl:id>
        <rdfs:label>Palaw Township</rdfs:label>
    </owl:NamedIndividual>
    


    <!-- http://purl.obolibrary.org/obo/GAZ_00118606 -->

    <owl:NamedIndividual rdf:about="http://purl.obolibrary.org/obo/GAZ_00118606">
        <obo:RO_0001025 rdf:resource="http://purl.obolibrary.org/obo/GAZ_00025531"/>
        <obo:IAO_0000115>A populated place. A township of Mandalay, the second capital city of Myanmar.</obo:IAO_0000115>
        <oboInOwl:hasOBONamespace>GAZ</oboInOwl:hasOBONamespace>
        <oboInOwl:id>GAZ:00118606</oboInOwl:id>
        <rdfs:label>Mahar Aung Myay Township</rdfs:label>
    </owl:NamedIndividual>
    


    <!-- http://purl.obolibrary.org/obo/GAZ_00118607 -->

    <owl:NamedIndividual rdf:about="http://purl.obolibrary.org/obo/GAZ_00118607">
        <obo:RO_0001025 rdf:resource="http://purl.obolibrary.org/obo/GAZ_00025531"/>
        <obo:IAO_0000115>A populated place. A township of Mandalay, the second capital city of Myanmar.</obo:IAO_0000115>
        <oboInOwl:hasOBONamespace>GAZ</oboInOwl:hasOBONamespace>
        <oboInOwl:id>GAZ:00118607</oboInOwl:id>
        <rdfs:label>Chan Aye Thar Zan Township</rdfs:label>
    </owl:NamedIndividual>
    


    <!-- http://purl.obolibrary.org/obo/GAZ_00118608 -->

    <owl:NamedIndividual rdf:about="http://purl.obolibrary.org/obo/GAZ_00118608">
        <obo:RO_0001025 rdf:resource="http://purl.obolibrary.org/obo/GAZ_00025531"/>
        <obo:IAO_0000115>A populated place. A township of Mandalay, the second capital city of Myanmar.</obo:IAO_0000115>
        <oboInOwl:hasOBONamespace>GAZ</oboInOwl:hasOBONamespace>
        <oboInOwl:id>GAZ:00118608</oboInOwl:id>
        <rdfs:label>PaTheinGyi Township</rdfs:label>
    </owl:NamedIndividual>
    


    <!-- http://purl.obolibrary.org/obo/GAZ_00118609 -->

    <owl:NamedIndividual rdf:about="http://purl.obolibrary.org/obo/GAZ_00118609">
        <obo:RO_0001025 rdf:resource="http://purl.obolibrary.org/obo/GAZ_00025531"/>
        <obo:IAO_0000115>A populated place. A township of Mandalay, the second capital city of Myanmar.</obo:IAO_0000115>
        <oboInOwl:hasOBONamespace>GAZ</oboInOwl:hasOBONamespace>
        <oboInOwl:id>GAZ:00118609</oboInOwl:id>
        <rdfs:label>Pyi Gyi Tan Kon Township</rdfs:label>
    </owl:NamedIndividual>
    


    <!-- http://purl.obolibrary.org/obo/GAZ_00118610 -->

    <owl:NamedIndividual rdf:about="http://purl.obolibrary.org/obo/GAZ_00118610">
        <obo:RO_0001025 rdf:resource="http://purl.obolibrary.org/obo/GAZ_00025531"/>
        <obo:IAO_0000115>A populated place. A township of Mandalay, the second capital city of Myanmar.</obo:IAO_0000115>
        <oboInOwl:hasOBONamespace>GAZ</oboInOwl:hasOBONamespace>
        <oboInOwl:id>GAZ:00118610</oboInOwl:id>
        <rdfs:label>Chan Mya Thar Si Township</rdfs:label>
    </owl:NamedIndividual>
    


    <!-- http://purl.obolibrary.org/obo/GAZ_00118611 -->

    <owl:NamedIndividual rdf:about="http://purl.obolibrary.org/obo/GAZ_00118611">
        <obo:RO_0001025 rdf:resource="http://purl.obolibrary.org/obo/GAZ_00025531"/>
        <obo:IAO_0000115>A populated place. A township of Mandalay, the second capital city of Myanmar.</obo:IAO_0000115>
        <oboInOwl:hasOBONamespace>GAZ</oboInOwl:hasOBONamespace>
        <oboInOwl:id>GAZ:00118611</oboInOwl:id>
        <rdfs:label>Aung Myay Thar Zan Township</rdfs:label>
    </owl:NamedIndividual>
    


    <!-- http://purl.obolibrary.org/obo/GAZ_00118612 -->

    <owl:NamedIndividual rdf:about="http://purl.obolibrary.org/obo/GAZ_00118612">
        <obo:RO_0001025 rdf:resource="http://purl.obolibrary.org/obo/GAZ_00025531"/>
        <obo:IAO_0000115>A populated place. A township of Mandalay, the second capital city of Myanmar.</obo:IAO_0000115>
        <oboInOwl:hasOBONamespace>GAZ</oboInOwl:hasOBONamespace>
        <oboInOwl:id>GAZ:00118612</oboInOwl:id>
        <rdfs:label>Amarapura Township</rdfs:label>
    </owl:NamedIndividual>
    


    <!-- http://purl.obolibrary.org/obo/GAZ_00118613 -->

    <owl:NamedIndividual rdf:about="http://purl.obolibrary.org/obo/GAZ_00118613">
        <obo:RO_0001025 rdf:resource="http://purl.obolibrary.org/obo/GAZ_00025535"/>
        <obo:IAO_0000115>A populated place. A township of Pyin Oo Lwin District in the Mandalay Division of Burma.</obo:IAO_0000115>
        <oboInOwl:hasOBONamespace>GAZ</oboInOwl:hasOBONamespace>
        <oboInOwl:id>GAZ:00118613</oboInOwl:id>
        <rdfs:label>Pyin Oo Lwin Township</rdfs:label>
    </owl:NamedIndividual>
    


    <!-- http://purl.obolibrary.org/obo/GAZ_00118614 -->

    <owl:NamedIndividual rdf:about="http://purl.obolibrary.org/obo/GAZ_00118614">
        <obo:RO_0001025 rdf:resource="http://purl.obolibrary.org/obo/GAZ_00025535"/>
        <obo:IAO_0000115>A populated place. A township of Pyin Oo Lwin District in the Mandalay Division of Burma.</obo:IAO_0000115>
        <oboInOwl:hasOBONamespace>GAZ</oboInOwl:hasOBONamespace>
        <oboInOwl:id>GAZ:00118614</oboInOwl:id>
        <rdfs:label>Singu Township</rdfs:label>
    </owl:NamedIndividual>
    


    <!-- http://purl.obolibrary.org/obo/GAZ_00118615 -->

    <owl:NamedIndividual rdf:about="http://purl.obolibrary.org/obo/GAZ_00118615">
        <obo:RO_0001025 rdf:resource="http://purl.obolibrary.org/obo/GAZ_00025535"/>
        <obo:IAO_0000115>A populated place. A township of Pyin Oo Lwin District in the Mandalay Division of Burma.</obo:IAO_0000115>
        <oboInOwl:hasOBONamespace>GAZ</oboInOwl:hasOBONamespace>
        <oboInOwl:id>GAZ:00118615</oboInOwl:id>
        <rdfs:label>Mogok Township</rdfs:label>
    </owl:NamedIndividual>
    


    <!-- http://purl.obolibrary.org/obo/GAZ_00118616 -->

    <owl:NamedIndividual rdf:about="http://purl.obolibrary.org/obo/GAZ_00118616">
        <obo:RO_0001025 rdf:resource="http://purl.obolibrary.org/obo/GAZ_00025535"/>
        <obo:IAO_0000115>A populated place. A township of Pyin Oo Lwin District in the Mandalay Division of Burma.</obo:IAO_0000115>
        <oboInOwl:hasOBONamespace>GAZ</oboInOwl:hasOBONamespace>
        <oboInOwl:id>GAZ:00118616</oboInOwl:id>
        <rdfs:label>Madaya Township</rdfs:label>
    </owl:NamedIndividual>
    


    <!-- http://purl.obolibrary.org/obo/GAZ_00118617 -->

    <owl:NamedIndividual rdf:about="http://purl.obolibrary.org/obo/GAZ_00118617">
        <obo:RO_0001025 rdf:resource="http://purl.obolibrary.org/obo/GAZ_00025535"/>
        <obo:IAO_0000115>A populated place. A township of Pyin Oo Lwin District in the Mandalay Division of Burma.</obo:IAO_0000115>
        <oboInOwl:hasOBONamespace>GAZ</oboInOwl:hasOBONamespace>
        <oboInOwl:id>GAZ:00118617</oboInOwl:id>
        <rdfs:label>Thabeikkyin Township</rdfs:label>
    </owl:NamedIndividual>
    


    <!-- http://purl.obolibrary.org/obo/GAZ_00118618 -->

    <owl:NamedIndividual rdf:about="http://purl.obolibrary.org/obo/GAZ_00118618">
        <obo:RO_0001025 rdf:resource="http://purl.obolibrary.org/obo/GAZ_00025530"/>
        <obo:IAO_0000115>A populated place. A township of Kyaukse District in the Mandalay Division of Burma.</obo:IAO_0000115>
        <oboInOwl:hasOBONamespace>GAZ</oboInOwl:hasOBONamespace>
        <oboInOwl:id>GAZ:00118618</oboInOwl:id>
        <rdfs:label>Sintgaing Township</rdfs:label>
    </owl:NamedIndividual>
    


    <!-- http://purl.obolibrary.org/obo/GAZ_00118619 -->

    <owl:NamedIndividual rdf:about="http://purl.obolibrary.org/obo/GAZ_00118619">
        <obo:RO_0001025 rdf:resource="http://purl.obolibrary.org/obo/GAZ_00025530"/>
        <obo:IAO_0000115>A populated place. A township of Kyaukse District in the Mandalay Division of Burma.</obo:IAO_0000115>
        <oboInOwl:hasOBONamespace>GAZ</oboInOwl:hasOBONamespace>
        <oboInOwl:id>GAZ:00118619</oboInOwl:id>
        <rdfs:label>Myittha Township</rdfs:label>
    </owl:NamedIndividual>
    


    <!-- http://purl.obolibrary.org/obo/GAZ_00118620 -->

    <owl:NamedIndividual rdf:about="http://purl.obolibrary.org/obo/GAZ_00118620">
        <obo:RO_0001025 rdf:resource="http://purl.obolibrary.org/obo/GAZ_00025530"/>
        <obo:IAO_0000115>A populated place. A township of Kyaukse District in the Mandalay Division of Burma.</obo:IAO_0000115>
        <oboInOwl:hasOBONamespace>GAZ</oboInOwl:hasOBONamespace>
        <oboInOwl:id>GAZ:00118620</oboInOwl:id>
        <rdfs:label>Tada-U Township</rdfs:label>
    </owl:NamedIndividual>
    


    <!-- http://purl.obolibrary.org/obo/GAZ_00118621 -->

    <owl:NamedIndividual rdf:about="http://purl.obolibrary.org/obo/GAZ_00118621">
        <obo:RO_0001025 rdf:resource="http://purl.obolibrary.org/obo/GAZ_00025530"/>
        <obo:IAO_0000115>A populated place. A township of Kyaukse District in the Mandalay Division of Burma.</obo:IAO_0000115>
        <oboInOwl:hasOBONamespace>GAZ</oboInOwl:hasOBONamespace>
        <oboInOwl:id>GAZ:00118621</oboInOwl:id>
        <rdfs:label>Kyaukse Township</rdfs:label>
    </owl:NamedIndividual>
    


    <!-- http://purl.obolibrary.org/obo/GAZ_00118622 -->

    <owl:NamedIndividual rdf:about="http://purl.obolibrary.org/obo/GAZ_00118622">
        <obo:RO_0001025 rdf:resource="http://purl.obolibrary.org/obo/GAZ_00025533"/>
        <obo:IAO_0000115>A populated place. A township of Myingyan District in the Mandalay Division of Burma.</obo:IAO_0000115>
        <oboInOwl:hasOBONamespace>GAZ</oboInOwl:hasOBONamespace>
        <oboInOwl:id>GAZ:00118622</oboInOwl:id>
        <rdfs:label>Myingyan Township</rdfs:label>
    </owl:NamedIndividual>
    


    <!-- http://purl.obolibrary.org/obo/GAZ_00118623 -->

    <owl:NamedIndividual rdf:about="http://purl.obolibrary.org/obo/GAZ_00118623">
        <obo:RO_0001025 rdf:resource="http://purl.obolibrary.org/obo/GAZ_00025533"/>
        <obo:IAO_0000115>A populated place. A township of Myingyan District in the Mandalay Division of Burma.</obo:IAO_0000115>
        <oboInOwl:hasOBONamespace>GAZ</oboInOwl:hasOBONamespace>
        <oboInOwl:id>GAZ:00118623</oboInOwl:id>
        <rdfs:label>Natogyi Township</rdfs:label>
    </owl:NamedIndividual>
    


    <!-- http://purl.obolibrary.org/obo/GAZ_00118624 -->

    <owl:NamedIndividual rdf:about="http://purl.obolibrary.org/obo/GAZ_00118624">
        <obo:RO_0001025 rdf:resource="http://purl.obolibrary.org/obo/GAZ_00025533"/>
        <obo:IAO_0000115>A populated place. A township of Myingyan District in the Mandalay Division of Burma.</obo:IAO_0000115>
        <oboInOwl:hasOBONamespace>GAZ</oboInOwl:hasOBONamespace>
        <oboInOwl:id>GAZ:00118624</oboInOwl:id>
        <rdfs:label>Nganzun Township</rdfs:label>
    </owl:NamedIndividual>
    


    <!-- http://purl.obolibrary.org/obo/GAZ_00118625 -->

    <owl:NamedIndividual rdf:about="http://purl.obolibrary.org/obo/GAZ_00118625">
        <obo:RO_0001025 rdf:resource="http://purl.obolibrary.org/obo/GAZ_00025533"/>
        <obo:IAO_0000115>A populated place. A township of Myingyan District in the Mandalay Division of Burma.</obo:IAO_0000115>
        <oboInOwl:hasOBONamespace>GAZ</oboInOwl:hasOBONamespace>
        <oboInOwl:id>GAZ:00118625</oboInOwl:id>
        <rdfs:label>Thaungtha Township</rdfs:label>
    </owl:NamedIndividual>
    


    <!-- http://purl.obolibrary.org/obo/GAZ_00118626 -->

    <owl:NamedIndividual rdf:about="http://purl.obolibrary.org/obo/GAZ_00118626">
        <obo:RO_0001025 rdf:resource="http://purl.obolibrary.org/obo/GAZ_00025533"/>
        <obo:IAO_0000115>A populated place. A township of Myingyan District in the Mandalay Division of Burma.</obo:IAO_0000115>
        <oboInOwl:hasOBONamespace>GAZ</oboInOwl:hasOBONamespace>
        <oboInOwl:id>GAZ:00118626</oboInOwl:id>
        <rdfs:label>Kyaukpadaung Township</rdfs:label>
    </owl:NamedIndividual>
    


    <!-- http://purl.obolibrary.org/obo/GAZ_00118627 -->

    <owl:NamedIndividual rdf:about="http://purl.obolibrary.org/obo/GAZ_00118627">
        <obo:RO_0001025 rdf:resource="http://purl.obolibrary.org/obo/GAZ_00025534"/>
        <obo:IAO_0000115>A populated place. A township of Nyaung-U District in the Mandalay Division of Burma.</obo:IAO_0000115>
        <oboInOwl:hasOBONamespace>GAZ</oboInOwl:hasOBONamespace>
        <oboInOwl:id>GAZ:00118627</oboInOwl:id>
        <rdfs:label>Nyaung-U Township</rdfs:label>
    </owl:NamedIndividual>
    


    <!-- http://purl.obolibrary.org/obo/GAZ_00118628 -->

    <owl:NamedIndividual rdf:about="http://purl.obolibrary.org/obo/GAZ_00118628">
        <obo:RO_0001025 rdf:resource="http://purl.obolibrary.org/obo/GAZ_00025536"/>
        <obo:IAO_0000115>A populated place. A township of Yamethin District in the Mandalay Division of Burma.</obo:IAO_0000115>
        <oboInOwl:hasOBONamespace>GAZ</oboInOwl:hasOBONamespace>
        <oboInOwl:id>GAZ:00118628</oboInOwl:id>
        <rdfs:label>Pyawbwe Township</rdfs:label>
    </owl:NamedIndividual>
    


    <!-- http://purl.obolibrary.org/obo/GAZ_00118629 -->

    <owl:NamedIndividual rdf:about="http://purl.obolibrary.org/obo/GAZ_00118629">
        <obo:RO_0001025 rdf:resource="http://purl.obolibrary.org/obo/GAZ_00025536"/>
        <obo:IAO_0000115>A populated place. A township of Yamethin District in the Mandalay Division of Burma.</obo:IAO_0000115>
        <oboInOwl:hasOBONamespace>GAZ</oboInOwl:hasOBONamespace>
        <oboInOwl:id>GAZ:00118629</oboInOwl:id>
        <rdfs:label>Yamethin Township</rdfs:label>
    </owl:NamedIndividual>
    


    <!-- http://purl.obolibrary.org/obo/GAZ_00118630 -->

    <owl:NamedIndividual rdf:about="http://purl.obolibrary.org/obo/GAZ_00118630">
        <obo:RO_0001025 rdf:resource="http://purl.obolibrary.org/obo/GAZ_00025536"/>
        <obo:IAO_0000115>A populated place. A township of Yamethin District in the Mandalay Division of Burma.</obo:IAO_0000115>
        <oboInOwl:hasOBONamespace>GAZ</oboInOwl:hasOBONamespace>
        <oboInOwl:id>GAZ:00118630</oboInOwl:id>
        <rdfs:label>Lewe Township</rdfs:label>
    </owl:NamedIndividual>
    


    <!-- http://purl.obolibrary.org/obo/GAZ_00118631 -->

    <owl:NamedIndividual rdf:about="http://purl.obolibrary.org/obo/GAZ_00118631">
        <obo:RO_0001025 rdf:resource="http://purl.obolibrary.org/obo/GAZ_00025536"/>
        <obo:IAO_0000115>A populated place. A township of Yamethin District in the Mandalay Division of Burma.</obo:IAO_0000115>
        <oboInOwl:hasOBONamespace>GAZ</oboInOwl:hasOBONamespace>
        <oboInOwl:id>GAZ:00118631</oboInOwl:id>
        <rdfs:label>Tatkon Township</rdfs:label>
    </owl:NamedIndividual>
    


    <!-- http://purl.obolibrary.org/obo/GAZ_00118632 -->

    <owl:NamedIndividual rdf:about="http://purl.obolibrary.org/obo/GAZ_00118632">
        <obo:RO_0001025 rdf:resource="http://purl.obolibrary.org/obo/GAZ_00025536"/>
        <obo:IAO_0000115>A populated place. A township of Yamethin District in the Mandalay Division of Burma.</obo:IAO_0000115>
        <oboInOwl:hasOBONamespace>GAZ</oboInOwl:hasOBONamespace>
        <oboInOwl:id>GAZ:00118632</oboInOwl:id>
        <rdfs:label>Pyinmana Township</rdfs:label>
    </owl:NamedIndividual>
    


    <!-- http://purl.obolibrary.org/obo/GAZ_00118633 -->

    <owl:NamedIndividual rdf:about="http://purl.obolibrary.org/obo/GAZ_00118633">
        <obo:RO_0001025 rdf:resource="http://purl.obolibrary.org/obo/GAZ_00025532"/>
        <obo:IAO_0000115>A populated place. A township of Meiktila District in the Mandalay Division of Burma.</obo:IAO_0000115>
        <oboInOwl:hasOBONamespace>GAZ</oboInOwl:hasOBONamespace>
        <oboInOwl:id>GAZ:00118633</oboInOwl:id>
        <rdfs:label>Mahlaing Township</rdfs:label>
    </owl:NamedIndividual>
    


    <!-- http://purl.obolibrary.org/obo/GAZ_00118634 -->

    <owl:NamedIndividual rdf:about="http://purl.obolibrary.org/obo/GAZ_00118634">
        <obo:RO_0001025 rdf:resource="http://purl.obolibrary.org/obo/GAZ_00025532"/>
        <obo:IAO_0000115>A populated place. A township of Meiktila District in the Mandalay Division of Burma.</obo:IAO_0000115>
        <oboInOwl:hasOBONamespace>GAZ</oboInOwl:hasOBONamespace>
        <oboInOwl:id>GAZ:00118634</oboInOwl:id>
        <rdfs:label>Thazi Township</rdfs:label>
    </owl:NamedIndividual>
    


    <!-- http://purl.obolibrary.org/obo/GAZ_00118635 -->

    <owl:NamedIndividual rdf:about="http://purl.obolibrary.org/obo/GAZ_00118635">
        <obo:RO_0001025 rdf:resource="http://purl.obolibrary.org/obo/GAZ_00025532"/>
        <obo:IAO_0000115>A populated place. A township of Meiktila District in the Mandalay Division of Burma.</obo:IAO_0000115>
        <oboInOwl:hasOBONamespace>GAZ</oboInOwl:hasOBONamespace>
        <oboInOwl:id>GAZ:00118635</oboInOwl:id>
        <rdfs:label>Wundwin Township</rdfs:label>
    </owl:NamedIndividual>
    


    <!-- http://purl.obolibrary.org/obo/GAZ_00118636 -->

    <owl:NamedIndividual rdf:about="http://purl.obolibrary.org/obo/GAZ_00118636">
        <obo:RO_0001025 rdf:resource="http://purl.obolibrary.org/obo/GAZ_00025532"/>
        <obo:IAO_0000115>A populated place. A township of Meiktila District in the Mandalay Division of Burma.</obo:IAO_0000115>
        <oboInOwl:hasOBONamespace>GAZ</oboInOwl:hasOBONamespace>
        <oboInOwl:id>GAZ:00118636</oboInOwl:id>
        <rdfs:label>Meiktila Township</rdfs:label>
    </owl:NamedIndividual>
    


    <!-- http://purl.obolibrary.org/obo/GAZ_00118637 -->

    <owl:NamedIndividual rdf:about="http://purl.obolibrary.org/obo/GAZ_00118637">
        <obo:RO_0001025 rdf:resource="http://purl.obolibrary.org/obo/GAZ_00118632"/>
        <obo:IAO_0000115>A reservoir in the Pyinmana Township of the Mandalay Division of central Burma. Constructed 1978-1987.</obo:IAO_0000115>
        <oboInOwl:hasOBONamespace>GAZ</oboInOwl:hasOBONamespace>
        <oboInOwl:id>GAZ:00118637</oboInOwl:id>
        <rdfs:label>Ngalaik Reservoir</rdfs:label>
    </owl:NamedIndividual>
    


    <!-- http://purl.obolibrary.org/obo/GAZ_00118638 -->

    <owl:NamedIndividual rdf:about="http://purl.obolibrary.org/obo/GAZ_00118638">
        <obo:RO_0001025 rdf:resource="http://purl.obolibrary.org/obo/GAZ_00025526"/>
        <obo:IAO_0000115>A populated place. A township of Yangon, the capital city of Burma. It is located in the eastern area of the city.</obo:IAO_0000115>
        <oboInOwl:hasOBONamespace>GAZ</oboInOwl:hasOBONamespace>
        <oboInOwl:id>GAZ:00118638</oboInOwl:id>
        <rdfs:label>Dagon Seikkan Township</rdfs:label>
    </owl:NamedIndividual>
    


    <!-- http://purl.obolibrary.org/obo/GAZ_00118639 -->

    <owl:NamedIndividual rdf:about="http://purl.obolibrary.org/obo/GAZ_00118639">
        <obo:RO_0001025 rdf:resource="http://purl.obolibrary.org/obo/GAZ_00025526"/>
        <obo:IAO_0000115>A populated place. A township of Yangon, the capital city of Burma. It is located in the eastern area of the city.</obo:IAO_0000115>
        <oboInOwl:hasOBONamespace>GAZ</oboInOwl:hasOBONamespace>
        <oboInOwl:id>GAZ:00118639</oboInOwl:id>
        <rdfs:label>North Okkalapa Township</rdfs:label>
    </owl:NamedIndividual>
    


    <!-- http://purl.obolibrary.org/obo/GAZ_00118640 -->

    <owl:NamedIndividual rdf:about="http://purl.obolibrary.org/obo/GAZ_00118640">
        <obo:RO_0001025 rdf:resource="http://purl.obolibrary.org/obo/GAZ_00025526"/>
        <obo:IAO_0000115>A populated place. A township of Yangon, the capital city of Burma. It is located in the eastern area of the city.</obo:IAO_0000115>
        <oboInOwl:hasOBONamespace>GAZ</oboInOwl:hasOBONamespace>
        <oboInOwl:id>GAZ:00118640</oboInOwl:id>
        <rdfs:label>Thingangyun Township</rdfs:label>
    </owl:NamedIndividual>
    


    <!-- http://purl.obolibrary.org/obo/GAZ_00118641 -->

    <owl:NamedIndividual rdf:about="http://purl.obolibrary.org/obo/GAZ_00118641">
        <obo:RO_0001025 rdf:resource="http://purl.obolibrary.org/obo/GAZ_00025526"/>
        <obo:IAO_0000115>A populated place. A township of Yangon, the capital city of Burma. It is located in the eastern area of the city.</obo:IAO_0000115>
        <oboInOwl:hasOBONamespace>GAZ</oboInOwl:hasOBONamespace>
        <oboInOwl:id>GAZ:00118641</oboInOwl:id>
        <rdfs:label>North Dagon Township</rdfs:label>
    </owl:NamedIndividual>
    


    <!-- http://purl.obolibrary.org/obo/GAZ_00118642 -->

    <owl:NamedIndividual rdf:about="http://purl.obolibrary.org/obo/GAZ_00118642">
        <obo:RO_0001025 rdf:resource="http://purl.obolibrary.org/obo/GAZ_00025526"/>
        <obo:IAO_0000115>A populated place. A township of Yangon, the capital city of Burma. It is located in the eastern area of the city.</obo:IAO_0000115>
        <oboInOwl:hasOBONamespace>GAZ</oboInOwl:hasOBONamespace>
        <oboInOwl:id>GAZ:00118642</oboInOwl:id>
        <rdfs:label>South Dagon Township</rdfs:label>
    </owl:NamedIndividual>
    


    <!-- http://purl.obolibrary.org/obo/GAZ_00118643 -->

    <owl:NamedIndividual rdf:about="http://purl.obolibrary.org/obo/GAZ_00118643">
        <obo:RO_0001025 rdf:resource="http://purl.obolibrary.org/obo/GAZ_00025526"/>
        <obo:IAO_0000115>A populated place. A township of Yangon, the capital city of Burma. It is located in the eastern area of the city.</obo:IAO_0000115>
        <oboInOwl:hasOBONamespace>GAZ</oboInOwl:hasOBONamespace>
        <oboInOwl:id>GAZ:00118643</oboInOwl:id>
        <rdfs:label>Botahtaung Township</rdfs:label>
    </owl:NamedIndividual>
    


    <!-- http://purl.obolibrary.org/obo/GAZ_00118644 -->

    <owl:NamedIndividual rdf:about="http://purl.obolibrary.org/obo/GAZ_00118644">
        <obo:RO_0001025 rdf:resource="http://purl.obolibrary.org/obo/GAZ_00025526"/>
        <obo:IAO_0000115>A populated place. A township or district of Yangon, the former capital city of Myanmar. It is located in the middle area of the city.</obo:IAO_0000115>
        <oboInOwl:hasOBONamespace>GAZ</oboInOwl:hasOBONamespace>
        <oboInOwl:id>GAZ:00118644</oboInOwl:id>
        <rdfs:label>Yankin Township</rdfs:label>
    </owl:NamedIndividual>
    


    <!-- http://purl.obolibrary.org/obo/GAZ_00118645 -->

    <owl:NamedIndividual rdf:about="http://purl.obolibrary.org/obo/GAZ_00118645">
        <obo:RO_0001025 rdf:resource="http://purl.obolibrary.org/obo/GAZ_00025526"/>
        <obo:IAO_0000115>A populated place. A township of Yangon, the capital city of Burma. It is located in the eastern area of the city.</obo:IAO_0000115>
        <oboInOwl:hasOBONamespace>GAZ</oboInOwl:hasOBONamespace>
        <oboInOwl:id>GAZ:00118645</oboInOwl:id>
        <rdfs:label>East Dagon Township</rdfs:label>
    </owl:NamedIndividual>
    


    <!-- http://purl.obolibrary.org/obo/GAZ_00118646 -->

    <owl:NamedIndividual rdf:about="http://purl.obolibrary.org/obo/GAZ_00118646">
        <obo:RO_0001025 rdf:resource="http://purl.obolibrary.org/obo/GAZ_00025526"/>
        <obo:IAO_0000115>A populated place. A township of Yangon, the capital city of Burma. It is located in the eastern area of the city.</obo:IAO_0000115>
        <oboInOwl:hasOBONamespace>GAZ</oboInOwl:hasOBONamespace>
        <oboInOwl:id>GAZ:00118646</oboInOwl:id>
        <rdfs:label>South Okkalapa Township</rdfs:label>
    </owl:NamedIndividual>
    


    <!-- http://purl.obolibrary.org/obo/GAZ_00118647 -->

    <owl:NamedIndividual rdf:about="http://purl.obolibrary.org/obo/GAZ_00118647">
        <obo:RO_0001025 rdf:resource="http://purl.obolibrary.org/obo/GAZ_00025526"/>
        <obo:IAO_0000115>A populated place. A township of Yangon, the capital city of Burma. It is located in the southern area of the city.</obo:IAO_0000115>
        <oboInOwl:hasOBONamespace>GAZ</oboInOwl:hasOBONamespace>
        <oboInOwl:id>GAZ:00118647</oboInOwl:id>
        <rdfs:label>Tamwe Township</rdfs:label>
    </owl:NamedIndividual>
    


    <!-- http://purl.obolibrary.org/obo/GAZ_00118648 -->

    <owl:NamedIndividual rdf:about="http://purl.obolibrary.org/obo/GAZ_00118648">
        <obo:RO_0001025 rdf:resource="http://purl.obolibrary.org/obo/GAZ_00025527"/>
        <obo:IAO_0000115>A populated place. A township of Yangon, the capital city of Burma. It is located in the western area of the city downtown.</obo:IAO_0000115>
        <oboInOwl:hasOBONamespace>GAZ</oboInOwl:hasOBONamespace>
        <oboInOwl:id>GAZ:00118648</oboInOwl:id>
        <rdfs:label>Bahan Township</rdfs:label>
    </owl:NamedIndividual>
    


    <!-- http://purl.obolibrary.org/obo/GAZ_00118649 -->

    <owl:NamedIndividual rdf:about="http://purl.obolibrary.org/obo/GAZ_00118649">
        <obo:RO_0001025 rdf:resource="http://purl.obolibrary.org/obo/GAZ_00025527"/>
        <obo:IAO_0000115>A populated place. A township of Yangon, the capital city of Burma. It is located in the western area of the city downtown.</obo:IAO_0000115>
        <oboInOwl:hasOBONamespace>GAZ</oboInOwl:hasOBONamespace>
        <oboInOwl:id>GAZ:00118649</oboInOwl:id>
        <rdfs:label>Kyauktada Township</rdfs:label>
    </owl:NamedIndividual>
    


    <!-- http://purl.obolibrary.org/obo/GAZ_00118650 -->

    <owl:NamedIndividual rdf:about="http://purl.obolibrary.org/obo/GAZ_00118650">
        <obo:RO_0001025 rdf:resource="http://purl.obolibrary.org/obo/GAZ_00025527"/>
        <obo:IAO_0000115>A populated place. A township of Yangon, the capital city of Burma. It is located in the western area of the city downtown.</obo:IAO_0000115>
        <oboInOwl:hasOBONamespace>GAZ</oboInOwl:hasOBONamespace>
        <oboInOwl:id>GAZ:00118650</oboInOwl:id>
        <rdfs:label>Seikkan Township</rdfs:label>
    </owl:NamedIndividual>
    


    <!-- http://purl.obolibrary.org/obo/GAZ_00118651 -->

    <owl:NamedIndividual rdf:about="http://purl.obolibrary.org/obo/GAZ_00118651">
        <obo:RO_0001025 rdf:resource="http://purl.obolibrary.org/obo/GAZ_00025527"/>
        <obo:IAO_0000115>A populated place. A township of Yangon, the capital city of Burma. It is located in the western area of the city downtown. Lanmadaw Township shares borders with Latha Township in the east, Ahlone Township in the west, Seikkan Township in the south, and Dagon Township in the north.</obo:IAO_0000115>
        <oboInOwl:hasOBONamespace>GAZ</oboInOwl:hasOBONamespace>
        <oboInOwl:id>GAZ:00118651</oboInOwl:id>
        <rdfs:label>Lanmadaw Township</rdfs:label>
    </owl:NamedIndividual>
    


    <!-- http://purl.obolibrary.org/obo/GAZ_00118652 -->

    <owl:NamedIndividual rdf:about="http://purl.obolibrary.org/obo/GAZ_00118652">
        <obo:RO_0001025 rdf:resource="http://purl.obolibrary.org/obo/GAZ_00025527"/>
        <obo:IAO_0000115>A populated place. A township of Yangon, the capital city of Burma. It is located in the western area of the city downtown.</obo:IAO_0000115>
        <oboInOwl:hasOBONamespace>GAZ</oboInOwl:hasOBONamespace>
        <oboInOwl:id>GAZ:00118652</oboInOwl:id>
        <rdfs:label>Sanchaung Township</rdfs:label>
    </owl:NamedIndividual>
    


    <!-- http://purl.obolibrary.org/obo/GAZ_00118653 -->

    <owl:NamedIndividual rdf:about="http://purl.obolibrary.org/obo/GAZ_00118653">
        <obo:RO_0001025 rdf:resource="http://purl.obolibrary.org/obo/GAZ_00025527"/>
        <obo:IAO_0000115>A populated place. A township of Yangon, the capital city of Burma. It is located in the western area of the city downtown.</obo:IAO_0000115>
        <oboInOwl:hasOBONamespace>GAZ</oboInOwl:hasOBONamespace>
        <oboInOwl:id>GAZ:00118653</oboInOwl:id>
        <rdfs:label>Dagon Township</rdfs:label>
    </owl:NamedIndividual>
    


    <!-- http://purl.obolibrary.org/obo/GAZ_00118654 -->

    <owl:NamedIndividual rdf:about="http://purl.obolibrary.org/obo/GAZ_00118654">
        <obo:RO_0001025 rdf:resource="http://purl.obolibrary.org/obo/GAZ_00025527"/>
        <obo:IAO_0000115>A populated place. A township of Yangon, the capital city of Burma. It is located in the western area of the city downtown.</obo:IAO_0000115>
        <oboInOwl:hasOBONamespace>GAZ</oboInOwl:hasOBONamespace>
        <oboInOwl:id>GAZ:00118654</oboInOwl:id>
        <rdfs:label>Kyeemyintdine Township</rdfs:label>
    </owl:NamedIndividual>
    


    <!-- http://purl.obolibrary.org/obo/GAZ_00118655 -->

    <owl:NamedIndividual rdf:about="http://purl.obolibrary.org/obo/GAZ_00118655">
        <obo:RO_0001025 rdf:resource="http://purl.obolibrary.org/obo/GAZ_00025527"/>
        <obo:IAO_0000115>A populated place. A township of Yangon, the capital city of Burma. It is located in the western area of the city downtown.</obo:IAO_0000115>
        <oboInOwl:hasOBONamespace>GAZ</oboInOwl:hasOBONamespace>
        <oboInOwl:id>GAZ:00118655</oboInOwl:id>
        <rdfs:label>Latha Township</rdfs:label>
    </owl:NamedIndividual>
    


    <!-- http://purl.obolibrary.org/obo/GAZ_00118656 -->

    <owl:NamedIndividual rdf:about="http://purl.obolibrary.org/obo/GAZ_00118656">
        <obo:RO_0001025 rdf:resource="http://purl.obolibrary.org/obo/GAZ_00025527"/>
        <obo:IAO_0000115>A populated place. A township of Yangon, the capital city of Burma. It is located in the western area of the city downtown.</obo:IAO_0000115>
        <oboInOwl:hasOBONamespace>GAZ</oboInOwl:hasOBONamespace>
        <oboInOwl:id>GAZ:00118656</oboInOwl:id>
        <rdfs:label>Ahlone Township</rdfs:label>
    </owl:NamedIndividual>
    


    <!-- http://purl.obolibrary.org/obo/GAZ_00118657 -->

    <owl:NamedIndividual rdf:about="http://purl.obolibrary.org/obo/GAZ_00118657">
        <obo:RO_0001025 rdf:resource="http://purl.obolibrary.org/obo/GAZ_00025527"/>
        <obo:IAO_0000115>A populated place. A township of Yangon, the capital city of Burma. It is located in the western area of the city downtown.</obo:IAO_0000115>
        <oboInOwl:hasOBONamespace>GAZ</oboInOwl:hasOBONamespace>
        <oboInOwl:id>GAZ:00118657</oboInOwl:id>
        <rdfs:label>Pabedan Township</rdfs:label>
    </owl:NamedIndividual>
    


    <!-- http://purl.obolibrary.org/obo/GAZ_00118658 -->

    <owl:NamedIndividual rdf:about="http://purl.obolibrary.org/obo/GAZ_00118658">
        <obo:RO_0001025 rdf:resource="http://purl.obolibrary.org/obo/GAZ_00025529"/>
        <obo:IAO_0000115>A populated place. A township or district of Yangon, the capital city of Burma. It is located in the northern area of the city.</obo:IAO_0000115>
        <oboInOwl:hasOBONamespace>GAZ</oboInOwl:hasOBONamespace>
        <oboInOwl:id>GAZ:00118658</oboInOwl:id>
        <rdfs:label>Insein Township</rdfs:label>
    </owl:NamedIndividual>
    


    <!-- http://purl.obolibrary.org/obo/GAZ_00118659 -->

    <owl:NamedIndividual rdf:about="http://purl.obolibrary.org/obo/GAZ_00118659">
        <obo:RO_0001025 rdf:resource="http://purl.obolibrary.org/obo/GAZ_00025529"/>
        <obo:IAO_0000115>A populated place. A township or district of Yangon, the capital city of Burma. It is located in the northern area of the city.</obo:IAO_0000115>
        <oboInOwl:hasOBONamespace>GAZ</oboInOwl:hasOBONamespace>
        <oboInOwl:id>GAZ:00118659</oboInOwl:id>
        <rdfs:label>Hlaingthaya Township</rdfs:label>
    </owl:NamedIndividual>
    


    <!-- http://purl.obolibrary.org/obo/GAZ_00118660 -->

    <owl:NamedIndividual rdf:about="http://purl.obolibrary.org/obo/GAZ_00118660">
        <obo:RO_0001025 rdf:resource="http://purl.obolibrary.org/obo/GAZ_00025529"/>
        <obo:IAO_0000115>A populated place. A township or district of Yangon, the capital city of Burma. It is located in the northern area of the city.</obo:IAO_0000115>
        <oboInOwl:hasOBONamespace>GAZ</oboInOwl:hasOBONamespace>
        <oboInOwl:id>GAZ:00118660</oboInOwl:id>
        <rdfs:label>Kamayut Township</rdfs:label>
    </owl:NamedIndividual>
    


    <!-- http://purl.obolibrary.org/obo/GAZ_00118661 -->

    <owl:NamedIndividual rdf:about="http://purl.obolibrary.org/obo/GAZ_00118661">
        <obo:RO_0001025 rdf:resource="http://purl.obolibrary.org/obo/GAZ_00025529"/>
        <obo:IAO_0000115>A populated place. A township or district of Yangon, the capital city of Burma. It is located in the northern area of the city.</obo:IAO_0000115>
        <oboInOwl:hasOBONamespace>GAZ</oboInOwl:hasOBONamespace>
        <oboInOwl:id>GAZ:00118661</oboInOwl:id>
        <rdfs:label>Pazundaung Township</rdfs:label>
    </owl:NamedIndividual>
    


    <!-- http://purl.obolibrary.org/obo/GAZ_00118662 -->

    <owl:NamedIndividual rdf:about="http://purl.obolibrary.org/obo/GAZ_00118662">
        <obo:RO_0001025 rdf:resource="http://purl.obolibrary.org/obo/GAZ_00025529"/>
        <obo:IAO_0000115>A populated place. A township or district of Yangon, the capital city of Burma. It is located in the northern area of the city.</obo:IAO_0000115>
        <oboInOwl:hasOBONamespace>GAZ</oboInOwl:hasOBONamespace>
        <oboInOwl:id>GAZ:00118662</oboInOwl:id>
        <rdfs:label>Mingaladon Township</rdfs:label>
    </owl:NamedIndividual>
    


    <!-- http://purl.obolibrary.org/obo/GAZ_00118663 -->

    <owl:NamedIndividual rdf:about="http://purl.obolibrary.org/obo/GAZ_00118663">
        <obo:RO_0001025 rdf:resource="http://purl.obolibrary.org/obo/GAZ_00025529"/>
        <obo:IAO_0000115>A populated place. A township or district of Yangon, the capital city of Burma. It is located in the northern area of the city.</obo:IAO_0000115>
        <oboInOwl:hasOBONamespace>GAZ</oboInOwl:hasOBONamespace>
        <oboInOwl:id>GAZ:00118663</oboInOwl:id>
        <rdfs:label>Mayangone Township</rdfs:label>
    </owl:NamedIndividual>
    


    <!-- http://purl.obolibrary.org/obo/GAZ_00118664 -->

    <owl:NamedIndividual rdf:about="http://purl.obolibrary.org/obo/GAZ_00118664">
        <obo:RO_0001025 rdf:resource="http://purl.obolibrary.org/obo/GAZ_00025529"/>
        <obo:IAO_0000115>A populated place. A township or district of Yangon, the capital city of Burma. It is located in the northern area of the city.</obo:IAO_0000115>
        <oboInOwl:hasOBONamespace>GAZ</oboInOwl:hasOBONamespace>
        <oboInOwl:id>GAZ:00118664</oboInOwl:id>
        <rdfs:label>Shwepyitha Township</rdfs:label>
    </owl:NamedIndividual>
    


    <!-- http://purl.obolibrary.org/obo/GAZ_00118665 -->

    <owl:NamedIndividual rdf:about="http://purl.obolibrary.org/obo/GAZ_00118665">
        <obo:RO_0001025 rdf:resource="http://purl.obolibrary.org/obo/GAZ_00025528"/>
        <obo:IAO_0000115>A populated place. A township of Yangon Division, the capital city of Burma. It is located in the southern area of the city.</obo:IAO_0000115>
        <oboInOwl:hasOBONamespace>GAZ</oboInOwl:hasOBONamespace>
        <oboInOwl:id>GAZ:00118665</oboInOwl:id>
        <rdfs:label>Dawbon Township</rdfs:label>
    </owl:NamedIndividual>
    


    <!-- http://purl.obolibrary.org/obo/GAZ_00118666 -->

    <owl:NamedIndividual rdf:about="http://purl.obolibrary.org/obo/GAZ_00118666">
        <obo:RO_0001025 rdf:resource="http://purl.obolibrary.org/obo/GAZ_00025528"/>
        <obo:IAO_0000115>A populated place. A township of Yangon Division, the capital city of Burma. It is located in the southern area of the city.</obo:IAO_0000115>
        <oboInOwl:hasOBONamespace>GAZ</oboInOwl:hasOBONamespace>
        <oboInOwl:id>GAZ:00118666</oboInOwl:id>
        <rdfs:label>Mingalataungnyunt Township</rdfs:label>
    </owl:NamedIndividual>
    


    <!-- http://purl.obolibrary.org/obo/GAZ_00118667 -->

    <owl:NamedIndividual rdf:about="http://purl.obolibrary.org/obo/GAZ_00118667">
        <obo:RO_0001025 rdf:resource="http://purl.obolibrary.org/obo/GAZ_00025528"/>
        <obo:IAO_0000115>A populated place. A township of Yangon Division, the capital city of Burma. It is located in the southern area of the city.</obo:IAO_0000115>
        <oboInOwl:hasOBONamespace>GAZ</oboInOwl:hasOBONamespace>
        <oboInOwl:id>GAZ:00118667</oboInOwl:id>
        <rdfs:label>Kungyangon Township</rdfs:label>
    </owl:NamedIndividual>
    


    <!-- http://purl.obolibrary.org/obo/GAZ_00118668 -->

    <owl:NamedIndividual rdf:about="http://purl.obolibrary.org/obo/GAZ_00118668">
        <obo:RO_0001025 rdf:resource="http://purl.obolibrary.org/obo/GAZ_00025528"/>
        <obo:IAO_0000115>A populated place. A township of Yangon Division, the capital city of Burma. It is located in the southern area of the city.</obo:IAO_0000115>
        <oboInOwl:hasOBONamespace>GAZ</oboInOwl:hasOBONamespace>
        <oboInOwl:id>GAZ:00118668</oboInOwl:id>
        <rdfs:label>Thaketa Township</rdfs:label>
    </owl:NamedIndividual>
    


    <!-- http://purl.obolibrary.org/obo/GAZ_00118669 -->

    <owl:NamedIndividual rdf:about="http://purl.obolibrary.org/obo/GAZ_00118669">
        <obo:RO_0001025 rdf:resource="http://purl.obolibrary.org/obo/GAZ_00025528"/>
        <obo:IAO_0000115>A populated place. A township of Yangon Division, the capital city of Burma. It is located in the southern area of the city.</obo:IAO_0000115>
        <oboInOwl:hasOBONamespace>GAZ</oboInOwl:hasOBONamespace>
        <oboInOwl:id>GAZ:00118669</oboInOwl:id>
        <rdfs:label>Seikkyi Kanaungto Township</rdfs:label>
    </owl:NamedIndividual>
    


    <!-- http://purl.obolibrary.org/obo/GAZ_00118670 -->

    <owl:NamedIndividual rdf:about="http://purl.obolibrary.org/obo/GAZ_00118670">
        <obo:RO_0001025 rdf:resource="http://purl.obolibrary.org/obo/GAZ_00025528"/>
        <obo:IAO_0000115>A populated place. A township of Yangon Division, the capital city of Burma. It is located in the southern area of the city.</obo:IAO_0000115>
        <oboInOwl:hasOBONamespace>GAZ</oboInOwl:hasOBONamespace>
        <oboInOwl:id>GAZ:00118670</oboInOwl:id>
        <rdfs:label>Dala Township</rdfs:label>
    </owl:NamedIndividual>
    


    <!-- http://purl.obolibrary.org/obo/GAZ_00147280 -->

    <owl:NamedIndividual rdf:about="http://purl.obolibrary.org/obo/GAZ_00147280">
        <rdf:type rdf:resource="http://purl.obolibrary.org/obo/ENVO_00000305"/>
        <obo:RO_0001025 rdf:resource="http://purl.obolibrary.org/obo/GAZ_00006899"/>
        <obo:IAO_0000115>A cape in Burma (Myanmar), 193 km from the Indian union territory of the Andaman and Nicobar Islands.</obo:IAO_0000115>
        <oboInOwl:hasOBONamespace>GAZ</oboInOwl:hasOBONamespace>
        <oboInOwl:id>GAZ:00147280</oboInOwl:id>
        <rdfs:label>Cape Negrais</rdfs:label>
    </owl:NamedIndividual>
    


    <!-- http://purl.obolibrary.org/obo/GAZ_00149198 -->

    <owl:NamedIndividual rdf:about="http://purl.obolibrary.org/obo/GAZ_00149198">
        <obo:RO_0001025 rdf:resource="http://purl.obolibrary.org/obo/GAZ_00056890"/>
        <obo:IAO_0000115>A subrange of the Patkai Hills, in Mizoram and partially in Tripura, India.</obo:IAO_0000115>
        <oboInOwl:hasOBONamespace>GAZ</oboInOwl:hasOBONamespace>
        <oboInOwl:id>GAZ:00149198</oboInOwl:id>
        <rdfs:label>Lushai Hills</rdfs:label>
    </owl:NamedIndividual>
    


    <!-- http://purl.obolibrary.org/obo/GAZ_00149246 -->

    <owl:NamedIndividual rdf:about="http://purl.obolibrary.org/obo/GAZ_00149246">
        <rdf:type rdf:resource="http://purl.obolibrary.org/obo/ENVO_00000106"/>
        <obo:RO_0001025 rdf:resource="http://purl.obolibrary.org/obo/GAZ_00056892"/>
        <obo:IAO_0000115>A range of hills that is part of the Garo-Khasi range in Meghalaya, India.</obo:IAO_0000115>
        <oboInOwl:hasOBONamespace>GAZ</oboInOwl:hasOBONamespace>
        <oboInOwl:id>GAZ:00149246</oboInOwl:id>
        <rdfs:label>Garo Hills</rdfs:label>
    </owl:NamedIndividual>
    


    <!-- http://purl.obolibrary.org/obo/GAZ_00149247 -->

    <owl:NamedIndividual rdf:about="http://purl.obolibrary.org/obo/GAZ_00149247">
        <rdf:type rdf:resource="http://purl.obolibrary.org/obo/ENVO_00000106"/>
        <obo:RO_0001025 rdf:resource="http://purl.obolibrary.org/obo/GAZ_00056892"/>
        <obo:IAO_0000115>A range of hills that is part of the Garo-Khasi range in Meghalaya, India, and is part of the Patkai range and of the Meghalaya subtropical forests ecoregion.</obo:IAO_0000115>
        <oboInOwl:hasOBONamespace>GAZ</oboInOwl:hasOBONamespace>
        <oboInOwl:id>GAZ:00149247</oboInOwl:id>
        <rdfs:label>Khasi Hills</rdfs:label>
    </owl:NamedIndividual>
    


    <!-- http://purl.obolibrary.org/obo/GAZ_00149248 -->

    <owl:NamedIndividual rdf:about="http://purl.obolibrary.org/obo/GAZ_00149248">
        <obo:RO_0001025 rdf:resource="http://purl.obolibrary.org/obo/GAZ_00056892"/>
        <oboInOwl:hasOBONamespace>GAZ</oboInOwl:hasOBONamespace>
        <oboInOwl:id>GAZ:00149248</oboInOwl:id>
        <rdfs:label>Jaintia Hills</rdfs:label>
    </owl:NamedIndividual>
    


    <!-- http://purl.obolibrary.org/obo/GAZ_00149697 -->

    <owl:NamedIndividual rdf:about="http://purl.obolibrary.org/obo/GAZ_00149697">
        <obo:RO_0001025 rdf:resource="http://purl.obolibrary.org/obo/GAZ_00149246"/>
        <obo:IAO_0000115>A national park located about 3,000 m above sea level, near the Garo Hills in Meghalaya.</obo:IAO_0000115>
        <oboInOwl:hasOBONamespace>GAZ</oboInOwl:hasOBONamespace>
        <oboInOwl:id>GAZ:00149697</oboInOwl:id>
        <rdfs:label>Balphakram National Park</rdfs:label>
    </owl:NamedIndividual>
    


    <!-- http://purl.obolibrary.org/obo/GAZ_00149698 -->

    <owl:NamedIndividual rdf:about="http://purl.obolibrary.org/obo/GAZ_00149698">
        <obo:RO_0001025 rdf:resource="http://purl.obolibrary.org/obo/GAZ_00056892"/>
        <obo:IAO_0000115>A national park located 2 km from Tura Peak in the Garo Hills district of Meghalaya, India.</obo:IAO_0000115>
        <oboInOwl:hasOBONamespace>GAZ</oboInOwl:hasOBONamespace>
        <oboInOwl:id>GAZ:00149698</oboInOwl:id>
        <rdfs:label>Nokrek National Park</rdfs:label>
    </owl:NamedIndividual>
    


    <!-- http://purl.obolibrary.org/obo/GAZ_00149772 -->

    <owl:NamedIndividual rdf:about="http://purl.obolibrary.org/obo/GAZ_00149772">
        <rdf:type rdf:resource="http://purl.obolibrary.org/obo/ENVO_00000106"/>
        <obo:IAO_0000115>A range of mountains reaching a height of around 3825 m, lie on the border of India and Myanmar. These hills are part of a complex mountain system, and the parts of the mountain ranges inside the Indian State of Nagaland are called Naga hills.</obo:IAO_0000115>
        <oboInOwl:hasOBONamespace>GAZ</oboInOwl:hasOBONamespace>
        <oboInOwl:id>GAZ:00149772</oboInOwl:id>
        <rdfs:label>Naga Hills</rdfs:label>
    </owl:NamedIndividual>
    


    <!-- http://purl.obolibrary.org/obo/GAZ_00224009 -->

    <owl:NamedIndividual rdf:about="http://purl.obolibrary.org/obo/GAZ_00224009">
        <obo:RO_0001025 rdf:resource="http://purl.obolibrary.org/obo/GAZ_00025513"/>
        <obo:IAO_0000115>A populated place. A township of Shwebo District.</obo:IAO_0000115>
        <oboInOwl:hasOBONamespace>GAZ</oboInOwl:hasOBONamespace>
        <oboInOwl:id>GAZ:00224009</oboInOwl:id>
        <rdfs:label>Kanbalu Township</rdfs:label>
    </owl:NamedIndividual>
    


    <!-- http://purl.obolibrary.org/obo/GAZ_00224010 -->

    <owl:NamedIndividual rdf:about="http://purl.obolibrary.org/obo/GAZ_00224010">
        <obo:RO_0001025 rdf:resource="http://purl.obolibrary.org/obo/GAZ_00025513"/>
        <oboInOwl:hasOBONamespace>GAZ</oboInOwl:hasOBONamespace>
        <oboInOwl:id>GAZ:00224010</oboInOwl:id>
        <rdfs:label>Khin-U Township</rdfs:label>
    </owl:NamedIndividual>
    


    <!-- http://purl.obolibrary.org/obo/GAZ_00224011 -->

    <owl:NamedIndividual rdf:about="http://purl.obolibrary.org/obo/GAZ_00224011">
        <obo:RO_0001025 rdf:resource="http://purl.obolibrary.org/obo/GAZ_00025513"/>
        <oboInOwl:hasOBONamespace>GAZ</oboInOwl:hasOBONamespace>
        <oboInOwl:id>GAZ:00224011</oboInOwl:id>
        <rdfs:label>Kyunhla Township</rdfs:label>
    </owl:NamedIndividual>
    


    <!-- http://purl.obolibrary.org/obo/GAZ_00224012 -->

    <owl:NamedIndividual rdf:about="http://purl.obolibrary.org/obo/GAZ_00224012">
        <obo:RO_0001025 rdf:resource="http://purl.obolibrary.org/obo/GAZ_00025513"/>
        <oboInOwl:hasOBONamespace>GAZ</oboInOwl:hasOBONamespace>
        <oboInOwl:id>GAZ:00224012</oboInOwl:id>
        <rdfs:label>Shwebo Township</rdfs:label>
    </owl:NamedIndividual>
    


    <!-- http://purl.obolibrary.org/obo/GAZ_00224013 -->

    <owl:NamedIndividual rdf:about="http://purl.obolibrary.org/obo/GAZ_00224013">
        <obo:RO_0001025 rdf:resource="http://purl.obolibrary.org/obo/GAZ_00025513"/>
        <oboInOwl:hasOBONamespace>GAZ</oboInOwl:hasOBONamespace>
        <oboInOwl:id>GAZ:00224013</oboInOwl:id>
        <rdfs:label>Taze Township</rdfs:label>
    </owl:NamedIndividual>
    


    <!-- http://purl.obolibrary.org/obo/GAZ_00224014 -->

    <owl:NamedIndividual rdf:about="http://purl.obolibrary.org/obo/GAZ_00224014">
        <obo:RO_0001025 rdf:resource="http://purl.obolibrary.org/obo/GAZ_00025513"/>
        <oboInOwl:hasOBONamespace>GAZ</oboInOwl:hasOBONamespace>
        <oboInOwl:id>GAZ:00224014</oboInOwl:id>
        <rdfs:label>Wetlet Township</rdfs:label>
    </owl:NamedIndividual>
    


    <!-- http://purl.obolibrary.org/obo/GAZ_00224015 -->

    <owl:NamedIndividual rdf:about="http://purl.obolibrary.org/obo/GAZ_00224015">
        <obo:RO_0001025 rdf:resource="http://purl.obolibrary.org/obo/GAZ_00025513"/>
        <oboInOwl:hasOBONamespace>GAZ</oboInOwl:hasOBONamespace>
        <oboInOwl:id>GAZ:00224015</oboInOwl:id>
        <rdfs:label>Ye-U Township</rdfs:label>
    </owl:NamedIndividual>
    


    <!-- http://purl.obolibrary.org/obo/GAZ_00247036 -->

    <owl:NamedIndividual rdf:about="http://purl.obolibrary.org/obo/GAZ_00247036">
        <obo:RO_0001025 rdf:resource="http://purl.obolibrary.org/obo/GAZ_02000012"/>
        <obo:IAO_0000115>A freshwater lake located 110 km WSW of Myitkyina, Kachin State.</obo:IAO_0000115>
        <oboInOwl:hasOBONamespace>GAZ</oboInOwl:hasOBONamespace>
        <oboInOwl:id>GAZ:00247036</oboInOwl:id>
        <rdfs:label>Indawngy Lake</rdfs:label>
    </owl:NamedIndividual>
    


    <!-- http://purl.obolibrary.org/obo/GAZ_00247037 -->

    <owl:NamedIndividual rdf:about="http://purl.obolibrary.org/obo/GAZ_00247037">
        <obo:RO_0001025 rdf:resource="http://purl.obolibrary.org/obo/GAZ_00224009"/>
        <obo:IAO_0000115>A protected area. Located approximately 180 km NNW of Mandalay in Kanbalu township, upper Sagaing Division. The sanctuary lies between the Mu and Irrawaddy Rivers. Incorporates Kyatthin Fuel Reserve and the Kyatthin Extension Reserve. Established 1941-06-19.</obo:IAO_0000115>
        <oboInOwl:hasOBONamespace>GAZ</oboInOwl:hasOBONamespace>
        <oboInOwl:id>GAZ:00247037</oboInOwl:id>
        <rdfs:label>Kyatthin Wildlife Sanctuary</rdfs:label>
    </owl:NamedIndividual>
    


    <!-- http://purl.obolibrary.org/obo/GAZ_00247039 -->

    <owl:NamedIndividual rdf:about="http://purl.obolibrary.org/obo/GAZ_00247039">
        <obo:RO_0001025 rdf:resource="http://purl.obolibrary.org/obo/GAZ_00247037"/>
        <obo:IAO_0000115>A protected area.</obo:IAO_0000115>
        <oboInOwl:hasOBONamespace>GAZ</oboInOwl:hasOBONamespace>
        <oboInOwl:id>GAZ:00247039</oboInOwl:id>
        <rdfs:label>Kyatthin Fuel Reserve</rdfs:label>
    </owl:NamedIndividual>
    


    <!-- http://purl.obolibrary.org/obo/GAZ_00247040 -->

    <owl:NamedIndividual rdf:about="http://purl.obolibrary.org/obo/GAZ_00247040">
        <obo:RO_0001025 rdf:resource="http://purl.obolibrary.org/obo/GAZ_00247037"/>
        <obo:IAO_0000115>A protected area.</obo:IAO_0000115>
        <oboInOwl:hasOBONamespace>GAZ</oboInOwl:hasOBONamespace>
        <oboInOwl:id>GAZ:00247040</oboInOwl:id>
        <rdfs:label>Kyatthin Extension Reserve</rdfs:label>
    </owl:NamedIndividual>
    


    <!-- http://purl.obolibrary.org/obo/GAZ_00247041 -->

    <owl:NamedIndividual rdf:about="http://purl.obolibrary.org/obo/GAZ_00247041">
        <obo:RO_0001025 rdf:resource="http://purl.obolibrary.org/obo/GAZ_02000007"/>
        <obo:IAO_0000115>A valley.</obo:IAO_0000115>
        <oboInOwl:hasOBONamespace>GAZ</oboInOwl:hasOBONamespace>
        <oboInOwl:id>GAZ:00247041</oboInOwl:id>
        <rdfs:label>Balu Chaung Valley</rdfs:label>
    </owl:NamedIndividual>
    


    <!-- http://purl.obolibrary.org/obo/GAZ_00247042 -->

    <owl:NamedIndividual rdf:about="http://purl.obolibrary.org/obo/GAZ_00247042">
        <obo:RO_0001025 rdf:resource="http://purl.obolibrary.org/obo/GAZ_00247041"/>
        <obo:IAO_0000115>A river.</obo:IAO_0000115>
        <oboInOwl:hasOBONamespace>GAZ</oboInOwl:hasOBONamespace>
        <oboInOwl:id>GAZ:00247042</oboInOwl:id>
        <rdfs:label>Balu River</rdfs:label>
    </owl:NamedIndividual>
    


    <!-- http://purl.obolibrary.org/obo/GAZ_00247043 -->

    <owl:NamedIndividual rdf:about="http://purl.obolibrary.org/obo/GAZ_00247043">
        <obo:RO_0001025 rdf:resource="http://purl.obolibrary.org/obo/GAZ_00247042"/>
        <obo:IAO_0000115>A dam. Impounds Mong Pai Lake. Constructed 1971-1972.</obo:IAO_0000115>
        <oboInOwl:hasOBONamespace>GAZ</oboInOwl:hasOBONamespace>
        <oboInOwl:id>GAZ:00247043</oboInOwl:id>
        <rdfs:label>Mong Pai Dam</rdfs:label>
    </owl:NamedIndividual>
    


    <!-- http://purl.obolibrary.org/obo/GAZ_00247044 -->

    <owl:NamedIndividual rdf:about="http://purl.obolibrary.org/obo/GAZ_00247044">
        <obo:RO_0001025 rdf:resource="http://purl.obolibrary.org/obo/GAZ_00247042"/>
        <obo:IAO_0000115>An artificial lake. Impounded by Mong Pai Dam. Constructed 1971-1972.</obo:IAO_0000115>
        <oboInOwl:hasOBONamespace>GAZ</oboInOwl:hasOBONamespace>
        <oboInOwl:id>GAZ:00247044</oboInOwl:id>
        <rdfs:label>Mong Pai Lake</rdfs:label>
    </owl:NamedIndividual>
    


    <!-- http://purl.obolibrary.org/obo/GAZ_00247045 -->

    <owl:NamedIndividual rdf:about="http://purl.obolibrary.org/obo/GAZ_00247045">
        <obo:RO_0001025 rdf:resource="http://purl.obolibrary.org/obo/GAZ_00247044"/>
        <obo:IAO_0000115>An island.</obo:IAO_0000115>
        <oboInOwl:hasOBONamespace>GAZ</oboInOwl:hasOBONamespace>
        <oboInOwl:id>GAZ:00247045</oboInOwl:id>
        <rdfs:label>Loi Pan Sone Island</rdfs:label>
    </owl:NamedIndividual>
    


    <!-- http://purl.obolibrary.org/obo/GAZ_00247046 -->

    <owl:NamedIndividual rdf:about="http://purl.obolibrary.org/obo/GAZ_00247046">
        <obo:RO_0001025 rdf:resource="http://purl.obolibrary.org/obo/GAZ_00247044"/>
        <obo:IAO_0000115>An island.</obo:IAO_0000115>
        <oboInOwl:hasOBONamespace>GAZ</oboInOwl:hasOBONamespace>
        <oboInOwl:id>GAZ:00247046</oboInOwl:id>
        <rdfs:label>Ho Tein uIsland</rdfs:label>
    </owl:NamedIndividual>
    


    <!-- http://purl.obolibrary.org/obo/GAZ_00247047 -->

    <owl:NamedIndividual rdf:about="http://purl.obolibrary.org/obo/GAZ_00247047">
        <obo:RO_0001025 rdf:resource="http://purl.obolibrary.org/obo/GAZ_00247044"/>
        <obo:IAO_0000115>An island.</obo:IAO_0000115>
        <oboInOwl:hasOBONamespace>GAZ</oboInOwl:hasOBONamespace>
        <oboInOwl:id>GAZ:00247047</oboInOwl:id>
        <rdfs:label>Lonka island</rdfs:label>
    </owl:NamedIndividual>
    


    <!-- http://purl.obolibrary.org/obo/GAZ_00247048 -->

    <owl:NamedIndividual rdf:about="http://purl.obolibrary.org/obo/GAZ_00247048">
        <obo:RO_0001025 rdf:resource="http://purl.obolibrary.org/obo/GAZ_02000005"/>
        <obo:IAO_0000115>A protected area. Located 1 km west of Salin Town and 50 km NNW of Minbu, Minbu District, Magway Division. The sanctuary comprises an oval lake of approximately 200 ha, featuring minor bays and indentations, and surrounded by marshes.</obo:IAO_0000115>
        <oboInOwl:hasOBONamespace>GAZ</oboInOwl:hasOBONamespace>
        <oboInOwl:id>GAZ:00247048</oboInOwl:id>
        <rdfs:label>Wethtigan Wildlife Sanctuary</rdfs:label>
    </owl:NamedIndividual>
    


    <!-- http://purl.obolibrary.org/obo/GAZ_00247049 -->

    <owl:NamedIndividual rdf:about="http://purl.obolibrary.org/obo/GAZ_00247049">
        <obo:RO_0001025 rdf:resource="http://purl.obolibrary.org/obo/GAZ_00006899"/>
        <obo:IAO_0000115>A water storage reservoir located 25 km NNE of Pegu, east of the Rangoon to Mandalay highway. Located in a flat area at the headwaters of the Zwebat Creek and Malaka Chaung, to provide water for a canal linking the Sittang and Pegu rivers. The bund is 5-9m high, with two sluices in the east draining into the canal and thence to the Sittang River. Constructed 1904.</obo:IAO_0000115>
        <oboInOwl:hasOBONamespace>GAZ</oboInOwl:hasOBONamespace>
        <oboInOwl:id>GAZ:00247049</oboInOwl:id>
        <rdfs:label>Mohingyi Lake</rdfs:label>
    </owl:NamedIndividual>
    


    <!-- http://purl.obolibrary.org/obo/GAZ_00247050 -->

    <owl:NamedIndividual rdf:about="http://purl.obolibrary.org/obo/GAZ_00247050">
        <obo:RO_0001025 rdf:resource="http://purl.obolibrary.org/obo/GAZ_00247051"/>
        <obo:IAO_0000115>A water storage reservoir located in the southwestern extremity of the Pegu Yoma hill range, near Taikkyi Township, 65 km north of Yangon, Yangon Division. Constructed 1940.</obo:IAO_0000115>
        <oboInOwl:hasOBONamespace>GAZ</oboInOwl:hasOBONamespace>
        <oboInOwl:id>GAZ:00247050</oboInOwl:id>
        <rdfs:label>Gyobyu Reservoir</rdfs:label>
    </owl:NamedIndividual>
    


    <!-- http://purl.obolibrary.org/obo/GAZ_00247051 -->

    <owl:NamedIndividual rdf:about="http://purl.obolibrary.org/obo/GAZ_00247051">
        <obo:RO_0001025 rdf:resource="http://purl.obolibrary.org/obo/GAZ_02000006"/>
        <obo:IAO_0000115>A river.</obo:IAO_0000115>
        <oboInOwl:hasOBONamespace>GAZ</oboInOwl:hasOBONamespace>
        <oboInOwl:id>GAZ:00247051</oboInOwl:id>
        <rdfs:label>Gyobyu Chaung</rdfs:label>
    </owl:NamedIndividual>
    


    <!-- http://purl.obolibrary.org/obo/GAZ_00247052 -->

    <owl:NamedIndividual rdf:about="http://purl.obolibrary.org/obo/GAZ_00247052">
        <obo:RO_0001025 rdf:resource="http://purl.obolibrary.org/obo/GAZ_02000006"/>
        <obo:IAO_0000115>A water storage reservoir located about 20 km north of Yangon and 6 km east of the Yangon River, Yangon Division.</obo:IAO_0000115>
        <oboInOwl:hasOBONamespace>GAZ</oboInOwl:hasOBONamespace>
        <oboInOwl:id>GAZ:00247052</oboInOwl:id>
        <rdfs:label>Hlawga Lake</rdfs:label>
    </owl:NamedIndividual>
    


    <!-- http://purl.obolibrary.org/obo/GAZ_00247053 -->

    <owl:NamedIndividual rdf:about="http://purl.obolibrary.org/obo/GAZ_00247053">
        <obo:RO_0001025 rdf:resource="http://purl.obolibrary.org/obo/GAZ_02000006"/>
        <obo:IAO_0000115>A wildlife park. Located SE of Hlawga Lake. Opened 1984.</obo:IAO_0000115>
        <oboInOwl:hasOBONamespace>GAZ</oboInOwl:hasOBONamespace>
        <oboInOwl:id>GAZ:00247053</oboInOwl:id>
        <rdfs:label>Hlawga Wildlife and Zoo Park</rdfs:label>
    </owl:NamedIndividual>
    


    <!-- http://purl.obolibrary.org/obo/GAZ_00247054 -->

    <owl:NamedIndividual rdf:about="http://purl.obolibrary.org/obo/GAZ_00247054">
        <obo:RO_0001025 rdf:resource="http://purl.obolibrary.org/obo/GAZ_00247053"/>
        <obo:IAO_0000115>A freshwater lake.</obo:IAO_0000115>
        <oboInOwl:hasOBONamespace>GAZ</oboInOwl:hasOBONamespace>
        <oboInOwl:id>GAZ:00247054</oboInOwl:id>
        <rdfs:label>Zokanok Lake</rdfs:label>
    </owl:NamedIndividual>
    


    <!-- http://purl.obolibrary.org/obo/GAZ_00247055 -->

    <owl:NamedIndividual rdf:about="http://purl.obolibrary.org/obo/GAZ_00247055">
        <obo:RO_0001025 rdf:resource="http://purl.obolibrary.org/obo/GAZ_00115117"/>
        <oboInOwl:hasOBONamespace>GAZ</oboInOwl:hasOBONamespace>
        <oboInOwl:id>GAZ:00247055</oboInOwl:id>
        <rdfs:label>Pathein River</rdfs:label>
    </owl:NamedIndividual>
    


    <!-- http://purl.obolibrary.org/obo/GAZ_00247056 -->

    <owl:NamedIndividual rdf:about="http://purl.obolibrary.org/obo/GAZ_00247056">
        <obo:RO_0001025 rdf:resource="http://purl.obolibrary.org/obo/GAZ_00115117"/>
        <obo:IAO_0000115>One of the major rivers of the Irrawaddy Delta discharging to the Bay of Bengal.</obo:IAO_0000115>
        <oboInOwl:hasOBONamespace>GAZ</oboInOwl:hasOBONamespace>
        <oboInOwl:id>GAZ:00247056</oboInOwl:id>
        <rdfs:label>Pyapon River</rdfs:label>
    </owl:NamedIndividual>
    


    <!-- http://purl.obolibrary.org/obo/GAZ_00247057 -->

    <owl:NamedIndividual rdf:about="http://purl.obolibrary.org/obo/GAZ_00247057">
        <obo:RO_0001025 rdf:resource="http://purl.obolibrary.org/obo/GAZ_00115117"/>
        <obo:IAO_0000115>One of the major rivers of the Irrawaddy Delta discharging to the Bay of Bengal.</obo:IAO_0000115>
        <oboInOwl:hasOBONamespace>GAZ</oboInOwl:hasOBONamespace>
        <oboInOwl:id>GAZ:00247057</oboInOwl:id>
        <rdfs:label>Bogale River</rdfs:label>
    </owl:NamedIndividual>
    


    <!-- http://purl.obolibrary.org/obo/GAZ_00247058 -->

    <owl:NamedIndividual rdf:about="http://purl.obolibrary.org/obo/GAZ_00247058">
        <obo:RO_0001025 rdf:resource="http://purl.obolibrary.org/obo/GAZ_00115117"/>
        <obo:IAO_0000115>One of the major rivers of the Irrawaddy Delta discharging to the Bay of Bengal.</obo:IAO_0000115>
        <oboInOwl:hasOBONamespace>GAZ</oboInOwl:hasOBONamespace>
        <oboInOwl:id>GAZ:00247058</oboInOwl:id>
        <rdfs:label>Toe River</rdfs:label>
    </owl:NamedIndividual>
    


    <!-- http://purl.obolibrary.org/obo/GAZ_00247059 -->

    <owl:NamedIndividual rdf:about="http://purl.obolibrary.org/obo/GAZ_00247059">
        <obo:RO_0001025 rdf:resource="http://purl.obolibrary.org/obo/GAZ_00115117"/>
        <obo:IAO_0000115>One of the major rivers of the Irrawaddy Delta discharging to the Bay of Bengal.</obo:IAO_0000115>
        <oboInOwl:hasOBONamespace>GAZ</oboInOwl:hasOBONamespace>
        <oboInOwl:id>GAZ:00247059</oboInOwl:id>
        <rdfs:label>Bassein River</rdfs:label>
    </owl:NamedIndividual>
    


    <!-- http://purl.obolibrary.org/obo/GAZ_00247060 -->

    <owl:NamedIndividual rdf:about="http://purl.obolibrary.org/obo/GAZ_00247060">
        <obo:RO_0001025 rdf:resource="http://purl.obolibrary.org/obo/GAZ_00115117"/>
        <obo:IAO_0000115>One of the major rivers of the Irrawaddy Delta discharging to the Bay of Bengal.</obo:IAO_0000115>
        <oboInOwl:hasOBONamespace>GAZ</oboInOwl:hasOBONamespace>
        <oboInOwl:id>GAZ:00247060</oboInOwl:id>
        <rdfs:label>Thetkethaung River</rdfs:label>
    </owl:NamedIndividual>
    


    <!-- http://purl.obolibrary.org/obo/GAZ_00247061 -->

    <owl:NamedIndividual rdf:about="http://purl.obolibrary.org/obo/GAZ_00247061">
        <obo:RO_0001025 rdf:resource="http://purl.obolibrary.org/obo/GAZ_00115117"/>
        <obo:IAO_0000115>One of the major rivers of the Irrawaddy Delta discharging to the Bay of Bengal.</obo:IAO_0000115>
        <oboInOwl:hasOBONamespace>GAZ</oboInOwl:hasOBONamespace>
        <oboInOwl:id>GAZ:00247061</oboInOwl:id>
        <rdfs:label>Ywe River</rdfs:label>
    </owl:NamedIndividual>
    


    <!-- http://purl.obolibrary.org/obo/GAZ_00247062 -->

    <owl:NamedIndividual rdf:about="http://purl.obolibrary.org/obo/GAZ_00247062">
        <obo:RO_0001025 rdf:resource="http://purl.obolibrary.org/obo/GAZ_00115117"/>
        <obo:IAO_0000115>One of the major rivers of the Irrawaddy Delta discharging to the Bay of Bengal.</obo:IAO_0000115>
        <oboInOwl:hasOBONamespace>GAZ</oboInOwl:hasOBONamespace>
        <oboInOwl:id>GAZ:00247062</oboInOwl:id>
        <rdfs:label>Pyamalaw River</rdfs:label>
    </owl:NamedIndividual>
    


    <!-- http://purl.obolibrary.org/obo/GAZ_00247063 -->

    <owl:NamedIndividual rdf:about="http://purl.obolibrary.org/obo/GAZ_00247063">
        <obo:RO_0001025 rdf:resource="http://purl.obolibrary.org/obo/GAZ_00115117"/>
        <obo:IAO_0000115>One of the major rivers of the Irrawaddy Delta discharging to the Bay of Bengal.</obo:IAO_0000115>
        <oboInOwl:hasOBONamespace>GAZ</oboInOwl:hasOBONamespace>
        <oboInOwl:id>GAZ:00247063</oboInOwl:id>
        <rdfs:label>China Bakir River</rdfs:label>
    </owl:NamedIndividual>
    


    <!-- http://purl.obolibrary.org/obo/GAZ_00247064 -->

    <owl:NamedIndividual rdf:about="http://purl.obolibrary.org/obo/GAZ_00247064">
        <obo:RO_0001025 rdf:resource="http://purl.obolibrary.org/obo/GAZ_02000006"/>
        <obo:IAO_0000115>A river formed by the confluence of the Pegu and Myitmaka rivers and is a marine estuary that runs from Yangon emptying into the Gulf of Martaban of the Andaman Sea. The Twante Canal connects the Yangon River with the Irrawaddy Delta.</obo:IAO_0000115>
        <oboInOwl:hasOBONamespace>GAZ</oboInOwl:hasOBONamespace>
        <oboInOwl:id>GAZ:00247064</oboInOwl:id>
        <rdfs:label>Rangoon River</rdfs:label>
    </owl:NamedIndividual>
    


    <!-- http://purl.obolibrary.org/obo/GAZ_00247065 -->

    <owl:NamedIndividual rdf:about="http://purl.obolibrary.org/obo/GAZ_00247065">
        <obo:RO_0001025 rdf:resource="http://purl.obolibrary.org/obo/GAZ_00115117"/>
        <obo:IAO_0000115>A canal that links Yangon with the western part of the Irrawaddy Delta.</obo:IAO_0000115>
        <oboInOwl:hasOBONamespace>GAZ</oboInOwl:hasOBONamespace>
        <oboInOwl:id>GAZ:00247065</oboInOwl:id>
        <rdfs:label>Twante Canal</rdfs:label>
    </owl:NamedIndividual>
    


    <!-- http://purl.obolibrary.org/obo/GAZ_00247066 -->

    <owl:NamedIndividual rdf:about="http://purl.obolibrary.org/obo/GAZ_00247066">
        <obo:RO_0001025 rdf:resource="http://purl.obolibrary.org/obo/GAZ_00115117"/>
        <obo:IAO_0000115>An island off the mouth of the Irrawaddy River.</obo:IAO_0000115>
        <oboInOwl:hasOBONamespace>GAZ</oboInOwl:hasOBONamespace>
        <oboInOwl:id>GAZ:00247066</oboInOwl:id>
        <rdfs:label>Kain Thaung Kyun</rdfs:label>
    </owl:NamedIndividual>
    


    <!-- http://purl.obolibrary.org/obo/GAZ_00247067 -->

    <owl:NamedIndividual rdf:about="http://purl.obolibrary.org/obo/GAZ_00247067">
        <obo:RO_0001025 rdf:resource="http://purl.obolibrary.org/obo/GAZ_00247071"/>
        <obo:IAO_0000115>An island off the mouth of the Bogale River. Located about 10 km off the coast of the Irrawaddy Delta.</obo:IAO_0000115>
        <oboInOwl:hasOBONamespace>GAZ</oboInOwl:hasOBONamespace>
        <oboInOwl:id>GAZ:00247067</oboInOwl:id>
        <rdfs:label>Kadonlay Kyun</rdfs:label>
    </owl:NamedIndividual>
    


    <!-- http://purl.obolibrary.org/obo/GAZ_00247068 -->

    <owl:NamedIndividual rdf:about="http://purl.obolibrary.org/obo/GAZ_00247068">
        <obo:RO_0001025 rdf:resource="http://purl.obolibrary.org/obo/GAZ_00115117"/>
        <obo:IAO_0000115>An island off the mouth of the Bogale River.</obo:IAO_0000115>
        <oboInOwl:hasOBONamespace>GAZ</oboInOwl:hasOBONamespace>
        <oboInOwl:id>GAZ:00247068</oboInOwl:id>
        <rdfs:label>Gayedgyi Kyun</rdfs:label>
    </owl:NamedIndividual>
    


    <!-- http://purl.obolibrary.org/obo/GAZ_00247069 -->

    <owl:NamedIndividual rdf:about="http://purl.obolibrary.org/obo/GAZ_00247069">
        <obo:RO_0001025 rdf:resource="http://purl.obolibrary.org/obo/GAZ_00115117"/>
        <obo:IAO_0000115>A protected area.</obo:IAO_0000115>
        <oboInOwl:hasOBONamespace>GAZ</oboInOwl:hasOBONamespace>
        <oboInOwl:id>GAZ:00247069</oboInOwl:id>
        <rdfs:label>Kyagan Kwinbauk Reserved Forest</rdfs:label>
    </owl:NamedIndividual>
    


    <!-- http://purl.obolibrary.org/obo/GAZ_00247070 -->

    <owl:NamedIndividual rdf:about="http://purl.obolibrary.org/obo/GAZ_00247070">
        <obo:RO_0001025 rdf:resource="http://purl.obolibrary.org/obo/GAZ_00115117"/>
        <oboInOwl:hasOBONamespace>GAZ</oboInOwl:hasOBONamespace>
        <oboInOwl:id>GAZ:00247070</oboInOwl:id>
        <rdfs:label>Pyinalan Reserved Forest</rdfs:label>
    </owl:NamedIndividual>
    


    <!-- http://purl.obolibrary.org/obo/GAZ_00247071 -->

    <owl:NamedIndividual rdf:about="http://purl.obolibrary.org/obo/GAZ_00247071">
        <obo:RO_0001025 rdf:resource="http://purl.obolibrary.org/obo/GAZ_00115117"/>
        <oboInOwl:hasOBONamespace>GAZ</oboInOwl:hasOBONamespace>
        <oboInOwl:id>GAZ:00247071</oboInOwl:id>
        <rdfs:label>Kadonkani Reserved Forest</rdfs:label>
    </owl:NamedIndividual>
    


    <!-- http://purl.obolibrary.org/obo/GAZ_00247072 -->

    <owl:NamedIndividual rdf:about="http://purl.obolibrary.org/obo/GAZ_00247072">
        <obo:RO_0001025 rdf:resource="http://purl.obolibrary.org/obo/GAZ_00115117"/>
        <oboInOwl:hasOBONamespace>GAZ</oboInOwl:hasOBONamespace>
        <oboInOwl:id>GAZ:00247072</oboInOwl:id>
        <rdfs:label>Kakayen Reserved Forest</rdfs:label>
    </owl:NamedIndividual>
    


    <!-- http://purl.obolibrary.org/obo/GAZ_00247073 -->

    <owl:NamedIndividual rdf:about="http://purl.obolibrary.org/obo/GAZ_00247073">
        <obo:RO_0001025 rdf:resource="http://purl.obolibrary.org/obo/GAZ_00115117"/>
        <oboInOwl:hasOBONamespace>GAZ</oboInOwl:hasOBONamespace>
        <oboInOwl:id>GAZ:00247073</oboInOwl:id>
        <rdfs:label>Meinmahla Reserved Forest</rdfs:label>
    </owl:NamedIndividual>
    


    <!-- http://purl.obolibrary.org/obo/GAZ_00247074 -->

    <owl:NamedIndividual rdf:about="http://purl.obolibrary.org/obo/GAZ_00247074">
        <obo:RO_0001025 rdf:resource="http://purl.obolibrary.org/obo/GAZ_00115117"/>
        <obo:IAO_0000115>An island located in the mouth of the Bogale and Kadonkani Rivers. An estuarine island in the delta of the Irrawaddy River, almost entirely comprised of alluvial deposits from the Bogale River.</obo:IAO_0000115>
        <oboInOwl:hasOBONamespace>GAZ</oboInOwl:hasOBONamespace>
        <oboInOwl:id>GAZ:00247074</oboInOwl:id>
        <rdfs:label>Meinmahla Kyun</rdfs:label>
    </owl:NamedIndividual>
    


    <!-- http://purl.obolibrary.org/obo/GAZ_00247075 -->

    <owl:NamedIndividual rdf:about="http://purl.obolibrary.org/obo/GAZ_00247075">
        <obo:RO_0001025 rdf:resource="http://purl.obolibrary.org/obo/GAZ_00115117"/>
        <obo:IAO_0000115>Island located off the eastern edge of the Irrawaddy Delta, opposite the mouth of the China Bakir River. A group of small islands and mudflats formed by the deposition of silt from the China Bakir River. The area is separated from the mainland by a long shallow inlet, which dries out at low tide.</obo:IAO_0000115>
        <oboInOwl:hasOBONamespace>GAZ</oboInOwl:hasOBONamespace>
        <oboInOwl:id>GAZ:00247075</oboInOwl:id>
        <rdfs:label>Letkokkon Islands</rdfs:label>
    </owl:NamedIndividual>
    


    <!-- http://purl.obolibrary.org/obo/GAZ_00247076 -->

    <owl:NamedIndividual rdf:about="http://purl.obolibrary.org/obo/GAZ_00247076">
        <obo:RO_0001025 rdf:resource="http://purl.obolibrary.org/obo/GAZ_00115117"/>
        <obo:RO_0001025 rdf:resource="http://purl.obolibrary.org/obo/GAZ_02000002"/>
        <obo:IAO_0000115>An island. Located about 10 km off the southern Arakan coast, opposite the mouth of the Bassein River.</obo:IAO_0000115>
        <oboInOwl:hasOBONamespace>GAZ</oboInOwl:hasOBONamespace>
        <oboInOwl:id>GAZ:00247076</oboInOwl:id>
        <rdfs:label>Thamihia Island</rdfs:label>
    </owl:NamedIndividual>
    


    <!-- http://purl.obolibrary.org/obo/GAZ_00247077 -->

    <owl:NamedIndividual rdf:about="http://purl.obolibrary.org/obo/GAZ_00247077">
        <obo:RO_0001025 rdf:resource="http://purl.obolibrary.org/obo/GAZ_00247076"/>
        <obo:IAO_0000115>A protected area. Established 1970-10.</obo:IAO_0000115>
        <oboInOwl:hasOBONamespace>GAZ</oboInOwl:hasOBONamespace>
        <oboInOwl:id>GAZ:00247077</oboInOwl:id>
        <rdfs:label>Thamihia Kyun (Diamond Island) Wildlife Sanctuary</rdfs:label>
    </owl:NamedIndividual>
    


    <!-- http://purl.obolibrary.org/obo/GAZ_00247078 -->

    <owl:NamedIndividual rdf:about="http://purl.obolibrary.org/obo/GAZ_00247078">
        <obo:RO_0001025 rdf:resource="http://purl.obolibrary.org/obo/GAZ_02000000"/>
        <obo:IAO_0000115>Three groups of small islands off the Tenasserim coast, lying on a north-south axis and stretching over some 70 km of sea.</obo:IAO_0000115>
        <oboInOwl:hasOBONamespace>GAZ</oboInOwl:hasOBONamespace>
        <oboInOwl:id>GAZ:00247078</oboInOwl:id>
        <rdfs:label>Moscos Islands</rdfs:label>
    </owl:NamedIndividual>
    


    <!-- http://purl.obolibrary.org/obo/GAZ_00247079 -->

    <owl:NamedIndividual rdf:about="http://purl.obolibrary.org/obo/GAZ_00247079">
        <obo:RO_0001025 rdf:resource="http://purl.obolibrary.org/obo/GAZ_00247078"/>
        <obo:IAO_0000115>A protected area. Established (as a Wildlife Sanctuary) 1927.</obo:IAO_0000115>
        <oboInOwl:hasOBONamespace>GAZ</oboInOwl:hasOBONamespace>
        <oboInOwl:id>GAZ:00247079</oboInOwl:id>
        <rdfs:label>Moscos Islands Wildlife Sanctuary</rdfs:label>
    </owl:NamedIndividual>
    


    <!-- http://purl.obolibrary.org/obo/GAZ_00247080 -->

    <owl:NamedIndividual rdf:about="http://purl.obolibrary.org/obo/GAZ_00247080">
        <rdf:type rdf:resource="http://purl.obolibrary.org/obo/ENVO_00000220"/>
        <obo:RO_0001025 rdf:resource="http://purl.obolibrary.org/obo/GAZ_00247079"/>
        <obo:IAO_0000115>An island group.</obo:IAO_0000115>
        <oboInOwl:hasOBONamespace>GAZ</oboInOwl:hasOBONamespace>
        <oboInOwl:id>GAZ:00247080</oboInOwl:id>
        <rdfs:label>Middle Moscos Islands</rdfs:label>
    </owl:NamedIndividual>
    


    <!-- http://purl.obolibrary.org/obo/GAZ_00247081 -->

    <owl:NamedIndividual rdf:about="http://purl.obolibrary.org/obo/GAZ_00247081">
        <rdf:type rdf:resource="http://purl.obolibrary.org/obo/ENVO_00000220"/>
        <obo:RO_0001025 rdf:resource="http://purl.obolibrary.org/obo/GAZ_00247079"/>
        <obo:IAO_0000115>An island group.</obo:IAO_0000115>
        <oboInOwl:hasOBONamespace>GAZ</oboInOwl:hasOBONamespace>
        <oboInOwl:id>GAZ:00247081</oboInOwl:id>
        <rdfs:label>South Moscos Islands</rdfs:label>
    </owl:NamedIndividual>
    


    <!-- http://purl.obolibrary.org/obo/GAZ_00247082 -->

    <owl:NamedIndividual rdf:about="http://purl.obolibrary.org/obo/GAZ_00247082">
        <rdf:type rdf:resource="http://purl.obolibrary.org/obo/ENVO_00000220"/>
        <obo:RO_0001025 rdf:resource="http://purl.obolibrary.org/obo/GAZ_00247079"/>
        <obo:IAO_0000115>An island group.</obo:IAO_0000115>
        <oboInOwl:hasOBONamespace>GAZ</oboInOwl:hasOBONamespace>
        <oboInOwl:id>GAZ:00247082</oboInOwl:id>
        <rdfs:label>North Moscos Islands</rdfs:label>
    </owl:NamedIndividual>
    


    <!-- http://purl.obolibrary.org/obo/GAZ_00247083 -->

    <owl:NamedIndividual rdf:about="http://purl.obolibrary.org/obo/GAZ_00247083">
        <obo:RO_0001025 rdf:resource="http://purl.obolibrary.org/obo/GAZ_00247081"/>
        <obo:IAO_0000115>An island.</obo:IAO_0000115>
        <oboInOwl:hasOBONamespace>GAZ</oboInOwl:hasOBONamespace>
        <oboInOwl:id>GAZ:00247083</oboInOwl:id>
        <rdfs:label>Auk Bok</rdfs:label>
    </owl:NamedIndividual>
    


    <!-- http://purl.obolibrary.org/obo/GAZ_00247720 -->

    <owl:NamedIndividual rdf:about="http://purl.obolibrary.org/obo/GAZ_00247720">
        <obo:RO_0001025 rdf:resource="http://purl.obolibrary.org/obo/GAZ_02000010"/>
        <obo:IAO_0000115>A bay.</obo:IAO_0000115>
        <oboInOwl:hasOBONamespace>GAZ</oboInOwl:hasOBONamespace>
        <oboInOwl:id>GAZ:00247720</oboInOwl:id>
        <rdfs:label>Combermere Bay</rdfs:label>
    </owl:NamedIndividual>
    


    <!-- http://purl.obolibrary.org/obo/GAZ_00247731 -->

    <owl:NamedIndividual rdf:about="http://purl.obolibrary.org/obo/GAZ_00247731">
        <rdf:type rdf:resource="http://purl.obolibrary.org/obo/ENVO_00000856"/>
        <obo:RO_0001025 rdf:resource="http://purl.obolibrary.org/obo/GAZ_00118492"/>
        <obo:IAO_0000115>A populated place. A town in Kyauktaw Township, Sittwe District, in the Rakhine State of western Burma, located on the right bank of the Kaladan River, just south of the border with Chin State.</obo:IAO_0000115>
        <oboInOwl:hasOBONamespace>GAZ</oboInOwl:hasOBONamespace>
        <oboInOwl:id>GAZ:00247731</oboInOwl:id>
        <rdfs:label>Ngame</rdfs:label>
    </owl:NamedIndividual>
    


    <!-- http://purl.obolibrary.org/obo/GAZ_00247732 -->

    <owl:NamedIndividual rdf:about="http://purl.obolibrary.org/obo/GAZ_00247732">
        <obo:RO_0001025 rdf:resource="http://purl.obolibrary.org/obo/GAZ_00118487"/>
        <obo:IAO_0000115>A populated place. The capital of Rakhine State, Myanmar (Burma). Sittwe, pronounced site-tway in the Rakhine language, is located on an estuarial island created at the confluence of the Kaladan, Myu, and Lemyo rivers emptying into the Bay of Bengal.</obo:IAO_0000115>
        <oboInOwl:hasOBONamespace>GAZ</oboInOwl:hasOBONamespace>
        <oboInOwl:id>GAZ:00247732</oboInOwl:id>
        <rdfs:label>Sittwe</rdfs:label>
    </owl:NamedIndividual>
    


    <!-- http://purl.obolibrary.org/obo/GAZ_00247733 -->

    <owl:NamedIndividual rdf:about="http://purl.obolibrary.org/obo/GAZ_00247733">
        <rdf:type rdf:resource="http://purl.obolibrary.org/obo/ENVO_00000475"/>
        <obo:IAO_0000115>An arm of the Andaman Sea in the southern part of Burma. The Salween and Sittang rivers empty into it.</obo:IAO_0000115>
        <oboInOwl:hasOBONamespace>GAZ</oboInOwl:hasOBONamespace>
        <oboInOwl:id>GAZ:00247733</oboInOwl:id>
        <rdfs:label>Gulf of Martaban</rdfs:label>
    </owl:NamedIndividual>
    


    <!-- http://purl.obolibrary.org/obo/GAZ_00247734 -->

    <owl:NamedIndividual rdf:about="http://purl.obolibrary.org/obo/GAZ_00247734">
        <rdf:type rdf:resource="http://purl.obolibrary.org/obo/ENVO_00000106"/>
        <obo:RO_0001025 rdf:resource="http://purl.obolibrary.org/obo/GAZ_00006899"/>
        <obo:IAO_0000115>A range of low mountains and uplands between the Irrawaddy and the Sittaung River in central Burma (Myanmar). The range runs from Mount Popa in the north to Singguttara Hill (Theingottara Hill) in the south. Both the Pegu River and the Sittaung River arise in the Pegu Range.</obo:IAO_0000115>
        <oboInOwl:hasOBONamespace>GAZ</oboInOwl:hasOBONamespace>
        <oboInOwl:id>GAZ:00247734</oboInOwl:id>
        <rdfs:label>Pegu Range</rdfs:label>
    </owl:NamedIndividual>
    


    <!-- http://purl.obolibrary.org/obo/GAZ_00247737 -->

    <owl:NamedIndividual rdf:about="http://purl.obolibrary.org/obo/GAZ_00247737">
        <obo:RO_0001025 rdf:resource="http://purl.obolibrary.org/obo/GAZ_02000004"/>
        <obo:IAO_0000115>A river in south central Myanmar in Bago Division. The river originates at the edge of the Shan Plateau southeast of Mandalay, and flows southward to the Gulf of Martaban.</obo:IAO_0000115>
        <oboInOwl:hasOBONamespace>GAZ</oboInOwl:hasOBONamespace>
        <oboInOwl:id>GAZ:00247737</oboInOwl:id>
        <rdfs:label>Sittaung River</rdfs:label>
    </owl:NamedIndividual>
    


    <!-- http://purl.obolibrary.org/obo/GAZ_00247743 -->

    <owl:NamedIndividual rdf:about="http://purl.obolibrary.org/obo/GAZ_00247743">
        <obo:RO_0001025 rdf:resource="http://purl.obolibrary.org/obo/GAZ_02000008"/>
        <obo:IAO_0000115>A river. A tributary of the Salween River in Burma.</obo:IAO_0000115>
        <oboInOwl:hasOBONamespace>GAZ</oboInOwl:hasOBONamespace>
        <oboInOwl:id>GAZ:00247743</oboInOwl:id>
        <rdfs:label>Dontham River</rdfs:label>
    </owl:NamedIndividual>
    


    <!-- http://purl.obolibrary.org/obo/GAZ_00247744 -->

    <owl:NamedIndividual rdf:about="http://purl.obolibrary.org/obo/GAZ_00247744">
        <obo:RO_0001025 rdf:resource="http://purl.obolibrary.org/obo/GAZ_02000008"/>
        <obo:IAO_0000115>A river. A tributary of the Salween River in Burma.</obo:IAO_0000115>
        <oboInOwl:hasOBONamespace>GAZ</oboInOwl:hasOBONamespace>
        <oboInOwl:id>GAZ:00247744</oboInOwl:id>
        <rdfs:label>Gyaing River</rdfs:label>
    </owl:NamedIndividual>
    


    <!-- http://purl.obolibrary.org/obo/GAZ_00247745 -->

    <owl:NamedIndividual rdf:about="http://purl.obolibrary.org/obo/GAZ_00247745">
        <obo:RO_0001025 rdf:resource="http://purl.obolibrary.org/obo/GAZ_00118478"/>
        <obo:RO_0001025 rdf:resource="http://purl.obolibrary.org/obo/GAZ_00247746"/>
        <obo:IAO_0000115>A populated place. A city situated 300 km south east of Yangon and 70 km south of Thaton, at the mouth of Thanlwin (Salween) river. Mawlamyaing is situated in the Salween River delta, where the mouth of the Salween is sheltered by Bilugyun Island as it enters the Gulf of Martaban and the Andaman Sea.</obo:IAO_0000115>
        <oboInOwl:hasOBONamespace>GAZ</oboInOwl:hasOBONamespace>
        <oboInOwl:id>GAZ:00247745</oboInOwl:id>
        <rdfs:label>Mawlamyine</rdfs:label>
    </owl:NamedIndividual>
    


    <!-- http://purl.obolibrary.org/obo/GAZ_00247746 -->

    <owl:NamedIndividual rdf:about="http://purl.obolibrary.org/obo/GAZ_00247746">
        <obo:IAO_0000115>The delta of the Salween River.</obo:IAO_0000115>
        <oboInOwl:hasOBONamespace>GAZ</oboInOwl:hasOBONamespace>
        <oboInOwl:id>GAZ:00247746</oboInOwl:id>
        <rdfs:label>Salween River Delta</rdfs:label>
    </owl:NamedIndividual>
    


    <!-- http://purl.obolibrary.org/obo/GAZ_00247747 -->

    <owl:NamedIndividual rdf:about="http://purl.obolibrary.org/obo/GAZ_00247747">
        <obo:RO_0001025 rdf:resource="http://purl.obolibrary.org/obo/GAZ_00025547"/>
        <obo:IAO_0000115>An island.</obo:IAO_0000115>
        <oboInOwl:hasOBONamespace>GAZ</oboInOwl:hasOBONamespace>
        <oboInOwl:id>GAZ:00247747</oboInOwl:id>
        <rdfs:label>Bilugyun Island</rdfs:label>
    </owl:NamedIndividual>
    


    <!-- http://purl.obolibrary.org/obo/GAZ_00247748 -->

    <owl:NamedIndividual rdf:about="http://purl.obolibrary.org/obo/GAZ_00247748">
        <obo:RO_0001025 rdf:resource="http://purl.obolibrary.org/obo/GAZ_00247737"/>
        <obo:IAO_0000115>An estuary.</obo:IAO_0000115>
        <oboInOwl:hasOBONamespace>GAZ</oboInOwl:hasOBONamespace>
        <oboInOwl:id>GAZ:00247748</oboInOwl:id>
        <rdfs:label>Sittaung River Estuary</rdfs:label>
    </owl:NamedIndividual>
    


    <!-- http://purl.obolibrary.org/obo/GAZ_00247749 -->

    <owl:NamedIndividual rdf:about="http://purl.obolibrary.org/obo/GAZ_00247749">
        <obo:RO_0001025 rdf:resource="http://purl.obolibrary.org/obo/GAZ_02000008"/>
        <obo:IAO_0000115>A river.</obo:IAO_0000115>
        <oboInOwl:hasOBONamespace>GAZ</oboInOwl:hasOBONamespace>
        <oboInOwl:id>GAZ:00247749</oboInOwl:id>
        <rdfs:label>Bilin River</rdfs:label>
    </owl:NamedIndividual>
    


    <!-- http://purl.obolibrary.org/obo/GAZ_00247750 -->

    <owl:NamedIndividual rdf:about="http://purl.obolibrary.org/obo/GAZ_00247750">
        <obo:RO_0001025 rdf:resource="http://purl.obolibrary.org/obo/GAZ_02000000"/>
        <obo:IAO_0000115>A protected area.</obo:IAO_0000115>
        <oboInOwl:hasOBONamespace>GAZ</oboInOwl:hasOBONamespace>
        <oboInOwl:id>GAZ:00247750</oboInOwl:id>
        <rdfs:label>Pakchan Reserved Forest</rdfs:label>
    </owl:NamedIndividual>
    


    <!-- http://purl.obolibrary.org/obo/GAZ_00251779 -->

    <owl:NamedIndividual rdf:about="http://purl.obolibrary.org/obo/GAZ_00251779">
        <obo:IAO_0000115>A river. A tributary of the Mekong River. It originates from the Northern mountainous region of Xiangkhoang Province and flows south through Vientiane Province joining the Mekong at Vientiane Capital.</obo:IAO_0000115>
        <oboInOwl:hasOBONamespace>GAZ</oboInOwl:hasOBONamespace>
        <oboInOwl:id>GAZ:00251779</oboInOwl:id>
        <rdfs:label>Nam Ngum</rdfs:label>
    </owl:NamedIndividual>
    


    <!-- http://purl.obolibrary.org/obo/GAZ_00251780 -->

    <owl:NamedIndividual rdf:about="http://purl.obolibrary.org/obo/GAZ_00251780">
        <obo:IAO_0000115>A river. A tributary of the Mekong River.</obo:IAO_0000115>
        <oboInOwl:hasOBONamespace>GAZ</oboInOwl:hasOBONamespace>
        <oboInOwl:id>GAZ:00251780</oboInOwl:id>
        <rdfs:label>Nam Lik</rdfs:label>
    </owl:NamedIndividual>
    


    <!-- http://purl.obolibrary.org/obo/GAZ_00251781 -->

    <owl:NamedIndividual rdf:about="http://purl.obolibrary.org/obo/GAZ_00251781">
        <obo:RO_0001025 rdf:resource="http://purl.obolibrary.org/obo/GAZ_00251779"/>
        <obo:IAO_0000115>A hydroelectric dam on the Nam Ngum River. Impounds Ang Nam Ngum. Completed 1971.</obo:IAO_0000115>
        <oboInOwl:hasOBONamespace>GAZ</oboInOwl:hasOBONamespace>
        <oboInOwl:id>GAZ:00251781</oboInOwl:id>
        <rdfs:label>Nam Ngum Dam</rdfs:label>
    </owl:NamedIndividual>
    


    <!-- http://purl.obolibrary.org/obo/GAZ_00251782 -->

    <owl:NamedIndividual rdf:about="http://purl.obolibrary.org/obo/GAZ_00251782">
        <obo:RO_0001025 rdf:resource="http://purl.obolibrary.org/obo/GAZ_00251779"/>
        <obo:IAO_0000115>A reservoir. Impounded by Nam Ngum Dam.</obo:IAO_0000115>
        <oboInOwl:hasOBONamespace>GAZ</oboInOwl:hasOBONamespace>
        <oboInOwl:id>GAZ:00251782</oboInOwl:id>
        <rdfs:label>Ang Nam Ngum</rdfs:label>
    </owl:NamedIndividual>
    


    <!-- http://purl.obolibrary.org/obo/GAZ_00251794 -->

    <owl:NamedIndividual rdf:about="http://purl.obolibrary.org/obo/GAZ_00251794">
        <obo:IAO_0000115>A hydro power project on the Nam Theun river in Laos. Completed 2009-10.</obo:IAO_0000115>
        <oboInOwl:hasOBONamespace>GAZ</oboInOwl:hasOBONamespace>
        <oboInOwl:id>GAZ:00251794</oboInOwl:id>
        <rdfs:label>Nam Theun II Dam</rdfs:label>
    </owl:NamedIndividual>
    


    <!-- http://purl.obolibrary.org/obo/GAZ_00251795 -->

    <owl:NamedIndividual rdf:about="http://purl.obolibrary.org/obo/GAZ_00251795">
        <obo:IAO_0000115>A river in northwest Laos.</obo:IAO_0000115>
        <oboInOwl:hasOBONamespace>GAZ</oboInOwl:hasOBONamespace>
        <oboInOwl:id>GAZ:00251795</oboInOwl:id>
        <rdfs:label>Nam Tha</rdfs:label>
    </owl:NamedIndividual>
    


    <!-- http://purl.obolibrary.org/obo/GAZ_00257198 -->

    <owl:NamedIndividual rdf:about="http://purl.obolibrary.org/obo/GAZ_00257198">
        <obo:IAO_0000115>A river that originates in Shan State, Burma. It flows down and across the Burma-Thailand border to Mae Ai district, Chiang Mai Province. Most of its length is in Chiang Rai Province passing the districts Mueang Chiang Rai, Mae Chan, Chiang Saen and Wiang Chai. It joins the Mekong River in Chiang Saen district.</obo:IAO_0000115>
        <oboInOwl:hasOBONamespace>GAZ</oboInOwl:hasOBONamespace>
        <oboInOwl:id>GAZ:00257198</oboInOwl:id>
        <rdfs:label>Kok River</rdfs:label>
    </owl:NamedIndividual>
    


    <!-- http://purl.obolibrary.org/obo/GAZ_00257225 -->

    <owl:NamedIndividual rdf:about="http://purl.obolibrary.org/obo/GAZ_00257225">
        <obo:RO_0001025 rdf:resource="http://purl.obolibrary.org/obo/GAZ_00257198"/>
        <obo:IAO_0000115>A river.</obo:IAO_0000115>
        <oboInOwl:hasOBONamespace>GAZ</oboInOwl:hasOBONamespace>
        <oboInOwl:id>GAZ:00257225</oboInOwl:id>
        <rdfs:label>Huai Luang</rdfs:label>
    </owl:NamedIndividual>
    


    <!-- http://purl.obolibrary.org/obo/GAZ_00257226 -->

    <owl:NamedIndividual rdf:about="http://purl.obolibrary.org/obo/GAZ_00257226">
        <obo:RO_0001025 rdf:resource="http://purl.obolibrary.org/obo/GAZ_00257198"/>
        <obo:IAO_0000115>A river.</obo:IAO_0000115>
        <oboInOwl:hasOBONamespace>GAZ</oboInOwl:hasOBONamespace>
        <oboInOwl:id>GAZ:00257226</oboInOwl:id>
        <rdfs:label>Huai Rong Boa</rdfs:label>
    </owl:NamedIndividual>
    


    <!-- http://purl.obolibrary.org/obo/GAZ_00257227 -->

    <owl:NamedIndividual rdf:about="http://purl.obolibrary.org/obo/GAZ_00257227">
        <obo:RO_0001025 rdf:resource="http://purl.obolibrary.org/obo/GAZ_00257198"/>
        <obo:IAO_0000115>A river.</obo:IAO_0000115>
        <oboInOwl:hasOBONamespace>GAZ</oboInOwl:hasOBONamespace>
        <oboInOwl:id>GAZ:00257227</oboInOwl:id>
        <rdfs:label>Nam Mae Sakun</rdfs:label>
    </owl:NamedIndividual>
    


    <!-- http://purl.obolibrary.org/obo/GAZ_00257570 -->

    <owl:NamedIndividual rdf:about="http://purl.obolibrary.org/obo/GAZ_00257570">
        <obo:RO_0001025 rdf:resource="http://purl.obolibrary.org/obo/GAZ_00257759"/>
        <obo:IAO_0000115>A resevoir.</obo:IAO_0000115>
        <oboInOwl:hasOBONamespace>GAZ</oboInOwl:hasOBONamespace>
        <oboInOwl:id>GAZ:00257570</oboInOwl:id>
        <rdfs:label>Lam Pao Reservoir</rdfs:label>
    </owl:NamedIndividual>
    


    <!-- http://purl.obolibrary.org/obo/GAZ_00257756 -->

    <owl:NamedIndividual rdf:about="http://purl.obolibrary.org/obo/GAZ_00257756">
        <obo:IAO_0000115>A dam located 5.5 km west of the confluence of the Mun and Mekong rivers in Ubon Ratchathani province, Thailand. Completed 1994.</obo:IAO_0000115>
        <oboInOwl:hasOBONamespace>GAZ</oboInOwl:hasOBONamespace>
        <oboInOwl:id>GAZ:00257756</oboInOwl:id>
        <rdfs:label>Pak Mun Dam</rdfs:label>
    </owl:NamedIndividual>
    


    <!-- http://purl.obolibrary.org/obo/GAZ_00257759 -->

    <owl:NamedIndividual rdf:about="http://purl.obolibrary.org/obo/GAZ_00257759">
        <obo:IAO_0000115>A river. A tributary of the Chi River in northeast Thailand. The river originates at the Nong Han Kumphawapi Lake in Udon Thani Province, from where it flows through Kalasin Province until it discharges to the Chi at the boundary between Kalasin and Roi Et Province.</obo:IAO_0000115>
        <oboInOwl:hasOBONamespace>GAZ</oboInOwl:hasOBONamespace>
        <oboInOwl:id>GAZ:00257759</oboInOwl:id>
        <rdfs:label>Pao River</rdfs:label>
    </owl:NamedIndividual>
    


    <!-- http://purl.obolibrary.org/obo/GAZ_00259001 -->

    <owl:NamedIndividual rdf:about="http://purl.obolibrary.org/obo/GAZ_00259001">
        <obo:IAO_0000115>A dam.</obo:IAO_0000115>
        <oboInOwl:hasOBONamespace>GAZ</oboInOwl:hasOBONamespace>
        <oboInOwl:id>GAZ:00259001</oboInOwl:id>
        <rdfs:label>Sirindhorn Dam</rdfs:label>
    </owl:NamedIndividual>
    


    <!-- http://purl.obolibrary.org/obo/GAZ_00259002 -->

    <owl:NamedIndividual rdf:about="http://purl.obolibrary.org/obo/GAZ_00259002">
        <obo:IAO_0000115>A reservoir. Impounded by Sirindhorn Dam.</obo:IAO_0000115>
        <oboInOwl:hasOBONamespace>GAZ</oboInOwl:hasOBONamespace>
        <oboInOwl:id>GAZ:00259002</oboInOwl:id>
        <rdfs:label>Sirindhorn Reservoir</rdfs:label>
    </owl:NamedIndividual>
    


    <!-- http://purl.obolibrary.org/obo/GAZ_00260460 -->

    <owl:NamedIndividual rdf:about="http://purl.obolibrary.org/obo/GAZ_00260460">
        <obo:IAO_0000115>A river.</obo:IAO_0000115>
        <oboInOwl:hasOBONamespace>GAZ</oboInOwl:hasOBONamespace>
        <oboInOwl:id>GAZ:00260460</oboInOwl:id>
        <rdfs:label>Co Chien River</rdfs:label>
    </owl:NamedIndividual>
    


    <!-- http://purl.obolibrary.org/obo/GAZ_00260461 -->

    <owl:NamedIndividual rdf:about="http://purl.obolibrary.org/obo/GAZ_00260461">
        <obo:RO_0001025 rdf:resource="http://purl.obolibrary.org/obo/GAZ_00260460"/>
        <obo:IAO_0000115>An island.</obo:IAO_0000115>
        <oboInOwl:hasOBONamespace>GAZ</oboInOwl:hasOBONamespace>
        <oboInOwl:id>GAZ:00260461</oboInOwl:id>
        <rdfs:label>An Binh Island</rdfs:label>
    </owl:NamedIndividual>
    


    <!-- http://purl.obolibrary.org/obo/GAZ_00260462 -->

    <owl:NamedIndividual rdf:about="http://purl.obolibrary.org/obo/GAZ_00260462">
        <obo:RO_0001025 rdf:resource="http://purl.obolibrary.org/obo/GAZ_00260460"/>
        <obo:IAO_0000115>An island.</obo:IAO_0000115>
        <oboInOwl:hasOBONamespace>GAZ</oboInOwl:hasOBONamespace>
        <oboInOwl:id>GAZ:00260462</oboInOwl:id>
        <rdfs:label>Binh Hoa Phuoc Island</rdfs:label>
    </owl:NamedIndividual>
    


    <!-- http://purl.obolibrary.org/obo/GAZ_00260617 -->

    <owl:NamedIndividual rdf:about="http://purl.obolibrary.org/obo/GAZ_00260617">
        <obo:IAO_0000115>A river. Discharges to the South China Sea.</obo:IAO_0000115>
        <oboInOwl:hasOBONamespace>GAZ</oboInOwl:hasOBONamespace>
        <oboInOwl:id>GAZ:00260617</oboInOwl:id>
        <rdfs:label>Song Cua Tieu</rdfs:label>
    </owl:NamedIndividual>
    


    <!-- http://purl.obolibrary.org/obo/GAZ_00260618 -->

    <owl:NamedIndividual rdf:about="http://purl.obolibrary.org/obo/GAZ_00260618">
        <obo:IAO_0000115>A river. Discharges to the South China Sea.</obo:IAO_0000115>
        <oboInOwl:hasOBONamespace>GAZ</oboInOwl:hasOBONamespace>
        <oboInOwl:id>GAZ:00260618</oboInOwl:id>
        <rdfs:label>Song Cua Dai</rdfs:label>
    </owl:NamedIndividual>
    


    <!-- http://purl.obolibrary.org/obo/GAZ_00260619 -->

    <owl:NamedIndividual rdf:about="http://purl.obolibrary.org/obo/GAZ_00260619">
        <obo:IAO_0000115>A river. Discharges to the South China Sea.</obo:IAO_0000115>
        <oboInOwl:hasOBONamespace>GAZ</oboInOwl:hasOBONamespace>
        <oboInOwl:id>GAZ:00260619</oboInOwl:id>
        <rdfs:label>Song Ba Lai</rdfs:label>
    </owl:NamedIndividual>
    


    <!-- http://purl.obolibrary.org/obo/GAZ_00260620 -->

    <owl:NamedIndividual rdf:about="http://purl.obolibrary.org/obo/GAZ_00260620">
        <obo:IAO_0000115>A river. Discharges to the South China Sea.</obo:IAO_0000115>
        <oboInOwl:hasOBONamespace>GAZ</oboInOwl:hasOBONamespace>
        <oboInOwl:id>GAZ:00260620</oboInOwl:id>
        <rdfs:label>Song Ham Luong</rdfs:label>
    </owl:NamedIndividual>
    


    <!-- http://purl.obolibrary.org/obo/GAZ_00260621 -->

    <owl:NamedIndividual rdf:about="http://purl.obolibrary.org/obo/GAZ_00260621">
        <obo:IAO_0000115>A river. Discharges to the South China Sea.</obo:IAO_0000115>
        <oboInOwl:hasOBONamespace>GAZ</oboInOwl:hasOBONamespace>
        <oboInOwl:id>GAZ:00260621</oboInOwl:id>
        <rdfs:label>Song Hau Giang</rdfs:label>
    </owl:NamedIndividual>
    


    <!-- http://purl.obolibrary.org/obo/GAZ_02000000 -->

    <owl:NamedIndividual rdf:about="http://purl.obolibrary.org/obo/GAZ_02000000"/>
    


    <!-- http://purl.obolibrary.org/obo/GAZ_02000001 -->

    <owl:NamedIndividual rdf:about="http://purl.obolibrary.org/obo/GAZ_02000001"/>
    


    <!-- http://purl.obolibrary.org/obo/GAZ_02000002 -->

    <owl:NamedIndividual rdf:about="http://purl.obolibrary.org/obo/GAZ_02000002"/>
    


    <!-- http://purl.obolibrary.org/obo/GAZ_02000003 -->

    <owl:NamedIndividual rdf:about="http://purl.obolibrary.org/obo/GAZ_02000003"/>
    


    <!-- http://purl.obolibrary.org/obo/GAZ_02000004 -->

    <owl:NamedIndividual rdf:about="http://purl.obolibrary.org/obo/GAZ_02000004"/>
    


    <!-- http://purl.obolibrary.org/obo/GAZ_02000005 -->

    <owl:NamedIndividual rdf:about="http://purl.obolibrary.org/obo/GAZ_02000005"/>
    


    <!-- http://purl.obolibrary.org/obo/GAZ_02000006 -->

    <owl:NamedIndividual rdf:about="http://purl.obolibrary.org/obo/GAZ_02000006"/>
    


    <!-- http://purl.obolibrary.org/obo/GAZ_02000007 -->

    <owl:NamedIndividual rdf:about="http://purl.obolibrary.org/obo/GAZ_02000007"/>
    


    <!-- http://purl.obolibrary.org/obo/GAZ_02000008 -->

    <owl:NamedIndividual rdf:about="http://purl.obolibrary.org/obo/GAZ_02000008"/>
    


    <!-- http://purl.obolibrary.org/obo/GAZ_02000009 -->

    <owl:NamedIndividual rdf:about="http://purl.obolibrary.org/obo/GAZ_02000009"/>
    


    <!-- http://purl.obolibrary.org/obo/GAZ_02000010 -->

    <owl:NamedIndividual rdf:about="http://purl.obolibrary.org/obo/GAZ_02000010"/>
    


    <!-- http://purl.obolibrary.org/obo/GAZ_02000011 -->

    <owl:NamedIndividual rdf:about="http://purl.obolibrary.org/obo/GAZ_02000011"/>
    


    <!-- http://purl.obolibrary.org/obo/GAZ_02000012 -->

    <owl:NamedIndividual rdf:about="http://purl.obolibrary.org/obo/GAZ_02000012"/>
    


    <!-- http://purl.obolibrary.org/obo/GAZ_02000013 -->

    <owl:NamedIndividual rdf:about="http://purl.obolibrary.org/obo/GAZ_02000013"/>
    


    <!-- http://purl.obolibrary.org/obo/GAZ_02000896 -->

    <owl:NamedIndividual rdf:about="http://purl.obolibrary.org/obo/GAZ_02000896">
        <obo:RO_0001025 rdf:resource="http://purl.obolibrary.org/obo/GAZ_00006899"/>
    </owl:NamedIndividual>
    


    <!-- 
    ///////////////////////////////////////////////////////////////////////////////////////
    //
    // Annotations
    //
    ///////////////////////////////////////////////////////////////////////////////////////
     -->

    <rdf:Description rdf:about="http://purl.obolibrary.org/obo/GAZ_00002782">
        <oboInOwl:hasOBONamespace>GAZ</oboInOwl:hasOBONamespace>
        <rdfs:label>Division (Myanmar)</rdfs:label>
        <oboInOwl:id>GAZ:00002782</oboInOwl:id>
    </rdf:Description>
    <rdf:Description rdf:about="http://purl.obolibrary.org/obo/GAZ_02000000">
        <rdfs:label>Tanintharyi Division</rdfs:label>
        <oboInOwl:id>GAZ:02000000</oboInOwl:id>
        <obo:IAO_0000115>A division of Myanmar, covering the long narrow southern part of the country on the Kra Isthmus. It borders the Andaman Sea to the west and Thailand to the east. To the north is the Mon State. The capital of the division is Dawei (Tavoy). The other main city is Mergui.</obo:IAO_0000115>
        <oboInOwl:hasOBONamespace>GAZ</oboInOwl:hasOBONamespace>
    </rdf:Description>
    <rdf:Description rdf:about="http://purl.obolibrary.org/obo/GAZ_02000001">
        <obo:IAO_0000115>An administrative division of Myanmar (Myanmar). It is located in the center of the country, bordering Sagaing Division and Magway Division to the west, Shan State to the east, and Bago Division and Kayin State to the south. The regional capital is Mandalay. In the south of the division lies the national capital of Naypyidaw, located in Pyinmana Township.</obo:IAO_0000115>
        <oboInOwl:id>GAZ:02000001</oboInOwl:id>
        <oboInOwl:hasOBONamespace>GAZ</oboInOwl:hasOBONamespace>
        <rdfs:label>Mandalay Division</rdfs:label>
    </rdf:Description>
    <rdf:Description rdf:about="http://purl.obolibrary.org/obo/GAZ_02000002">
        <obo:IAO_0000115>An administrative division of Myanmar, occupying the delta region of the Ayeyarwady River (also known as the Irrawaddy River). It is bordered by Bago Division to the north, Bago Division and Yangon Division to the east, and the Bay of Bengal to the south and west. It is contiguous with the Rakhine State in the northwest.</obo:IAO_0000115>
        <oboInOwl:id>GAZ:02000002</oboInOwl:id>
        <oboInOwl:hasOBONamespace>GAZ</oboInOwl:hasOBONamespace>
        <rdfs:label>Ayeyarwady Division</rdfs:label>
    </rdf:Description>
    <rdf:Description rdf:about="http://purl.obolibrary.org/obo/GAZ_02000003">
        <obo:IAO_0000115>An administrative division of Myanmar, located in the north-western part of the country. It is bordered by India&apos;s Nagaland and Manipur States to the north, Kachin State, Shan State, and Mandalay Division to the east, Mandalay Division and Magway Division to the south, with the Ayeyarwady River forming a greater part of its eastern and also southern boundary, and Chin State and India to the west.</obo:IAO_0000115>
        <oboInOwl:id>GAZ:02000003</oboInOwl:id>
        <rdfs:label>Sagaing Division</rdfs:label>
        <oboInOwl:hasOBONamespace>GAZ</oboInOwl:hasOBONamespace>
    </rdf:Description>
    <rdf:Description rdf:about="http://purl.obolibrary.org/obo/GAZ_02000004">
        <obo:IAO_0000115>An administrative division of Myanmar, located in the southern portion of the country. It is bordered by Magway Division and Mandalay Division to the north; Kayin State, Mon State and the Gulf of Martaban to the east; Yangon Division to the south and Ayeyarwady Division and Rakhine State to the west.</obo:IAO_0000115>
        <oboInOwl:id>GAZ:02000004</oboInOwl:id>
        <rdfs:label>Bago Division</rdfs:label>
        <oboInOwl:hasOBONamespace>GAZ</oboInOwl:hasOBONamespace>
    </rdf:Description>
    <rdf:Description rdf:about="http://purl.obolibrary.org/obo/GAZ_02000005">
        <obo:IAO_0000115>A division located in central Myanmar. It is bordered by Sagaing Division to the north, Mandalay Division to the east, Bago Division to the south, and Rakhine State and Chin State to the west.</obo:IAO_0000115>
        <rdfs:label>Magway Division</rdfs:label>
        <oboInOwl:id>GAZ:02000005</oboInOwl:id>
        <oboInOwl:hasOBONamespace>GAZ</oboInOwl:hasOBONamespace>
    </rdf:Description>
    <rdf:Description rdf:about="http://purl.obolibrary.org/obo/GAZ_02000006">
        <rdfs:label>Yangon Division</rdfs:label>
        <obo:IAO_0000115>An administrative division of Myanmar. It is bordered by Bago Division in the north and east, the Gulf of Mottama in the south, and Ayeyarwady Division in the west.</obo:IAO_0000115>
        <oboInOwl:hasOBONamespace>GAZ</oboInOwl:hasOBONamespace>
        <oboInOwl:id>GAZ:02000006</oboInOwl:id>
    </rdf:Description>
    <rdf:Description rdf:about="http://purl.obolibrary.org/obo/GAZ_02000007">
        <oboInOwl:hasOBONamespace>GAZ</oboInOwl:hasOBONamespace>
        <obo:IAO_0000115>An administrative division of Myanmar (Burma). Shan State borders China to the north, Laos to the east, and Thailand to the south. It also shares borders with five administrative divisions of Myanmar.</obo:IAO_0000115>
        <oboInOwl:id>GAZ:02000007</oboInOwl:id>
        <rdfs:label>Shan State</rdfs:label>
    </rdf:Description>
    <rdf:Description rdf:about="http://purl.obolibrary.org/obo/GAZ_02000008">
        <oboInOwl:hasOBONamespace>GAZ</oboInOwl:hasOBONamespace>
        <obo:IAO_0000115>An administrative division of Myanmar. It is sandwiched between Kayin State on the east, the Andaman Sea on the west, Bago Division on the north and Tanintharyi Division on the south. It has a short border with Thailand&apos;s Kanchanaburi Province at its south-eastern tip.</obo:IAO_0000115>
        <rdfs:label>Mon State</rdfs:label>
        <oboInOwl:id>GAZ:02000008</oboInOwl:id>
    </rdf:Description>
    <rdf:Description rdf:about="http://purl.obolibrary.org/obo/GAZ_02000009">
        <obo:IAO_0000115>An administrative division of Myanmar and also known as Karen State. The capital city is Pa-an.</obo:IAO_0000115>
        <oboInOwl:id>GAZ:02000009</oboInOwl:id>
        <rdfs:label>Kayin State</rdfs:label>
        <oboInOwl:hasOBONamespace>GAZ</oboInOwl:hasOBONamespace>
    </rdf:Description>
    <rdf:Description rdf:about="http://purl.obolibrary.org/obo/GAZ_02000010">
        <oboInOwl:id>GAZ:02000010</oboInOwl:id>
        <obo:IAO_0000115>A State of Myanmar. Situated the western coast, it is bordered by Chin State in the north, Magway Division, Bago Division and Ayeyarwady Division in the east, the Bay of Bengal to the west, and the Chittagong Division of Bangladesh to the northwest.</obo:IAO_0000115>
        <oboInOwl:hasOBONamespace>GAZ</oboInOwl:hasOBONamespace>
        <rdfs:label>Rakhine State</rdfs:label>
    </rdf:Description>
    <rdf:Description rdf:about="http://purl.obolibrary.org/obo/GAZ_02000011">
        <oboInOwl:id>GAZ:02000011</oboInOwl:id>
        <rdfs:label>Kayah State</rdfs:label>
        <oboInOwl:hasOBONamespace>GAZ</oboInOwl:hasOBONamespace>
        <obo:IAO_0000115>A State of Myanmar. Situated in eastern Myanmar, it is bounded on the north by Shan State, on the east by Thailand&apos;s Mae Hong Son Province, and on the south and west by Kayin State.</obo:IAO_0000115>
    </rdf:Description>
    <rdf:Description rdf:about="http://purl.obolibrary.org/obo/GAZ_02000012">
        <obo:IAO_0000115>The northernmost State of Burma. It is bordered by China to the north and east; Shan State to the south; and Sagaing Division and India to the west.</obo:IAO_0000115>
        <oboInOwl:id>GAZ:02000012</oboInOwl:id>
        <rdfs:label>Kachin State</rdfs:label>
        <oboInOwl:hasOBONamespace>GAZ</oboInOwl:hasOBONamespace>
    </rdf:Description>
    <rdf:Description rdf:about="http://purl.obolibrary.org/obo/GAZ_02000013">
        <obo:IAO_0000115>A state located in the western sector of Burma (Union of Myanmar). Its capital is Hakha.</obo:IAO_0000115>
        <rdfs:label>Chin State</rdfs:label>
        <oboInOwl:id>GAZ:02000013</oboInOwl:id>
        <oboInOwl:hasOBONamespace>GAZ</oboInOwl:hasOBONamespace>
    </rdf:Description>
    <rdf:Description rdf:about="http://purl.obolibrary.org/obo/GAZ_02000896">
        <oboInOwl:hasOBONamespace>GAZ</oboInOwl:hasOBONamespace>
        <oboInOwl:id>GAZ:02000896</oboInOwl:id>
        <rdfs:label>State (Myanmar)</rdfs:label>
    </rdf:Description>
</rdf:RDF>



<!-- Generated by the OWL API (version 4.5.6) https://github.com/owlcs/owlapi -->

