<?xml version="1.0"?>
<rdf:RDF xmlns="http://purl.obolibrary.org/obo/gaz/subsets/countries/Namibia.owl#"
     xml:base="http://purl.obolibrary.org/obo/gaz/subsets/countries/Namibia.owl"
     xmlns:obo="http://purl.obolibrary.org/obo/"
     xmlns:owl="http://www.w3.org/2002/07/owl#"
     xmlns:rdf="http://www.w3.org/1999/02/22-rdf-syntax-ns#"
     xmlns:xml="http://www.w3.org/XML/1998/namespace"
     xmlns:xsd="http://www.w3.org/2001/XMLSchema#"
     xmlns:rdfs="http://www.w3.org/2000/01/rdf-schema#"
     xmlns:oboInOwl="http://www.geneontology.org/formats/oboInOwl#">
    <owl:Ontology rdf:about="http://purl.obolibrary.org/obo/gaz/subsets/countries/Namibia.owl">
        <owl:imports rdf:resource="http://purl.obolibrary.org/obo/gaz/imports/envo_import.owl"/>
        <owl:imports rdf:resource="http://purl.obolibrary.org/obo/gaz/imports/ro_import.owl"/>
    </owl:Ontology>
    


    <!-- 
    ///////////////////////////////////////////////////////////////////////////////////////
    //
    // Annotation properties
    //
    ///////////////////////////////////////////////////////////////////////////////////////
     -->

    


    <!-- http://purl.obolibrary.org/obo/IAO_0000115 -->

    <owl:AnnotationProperty rdf:about="http://purl.obolibrary.org/obo/IAO_0000115"/>
    


    <!-- http://www.geneontology.org/formats/oboInOwl#hasOBONamespace -->

    <owl:AnnotationProperty rdf:about="http://www.geneontology.org/formats/oboInOwl#hasOBONamespace"/>
    


    <!-- http://www.geneontology.org/formats/oboInOwl#id -->

    <owl:AnnotationProperty rdf:about="http://www.geneontology.org/formats/oboInOwl#id"/>
    


    <!-- 
    ///////////////////////////////////////////////////////////////////////////////////////
    //
    // Object Properties
    //
    ///////////////////////////////////////////////////////////////////////////////////////
     -->

    


    <!-- http://purl.obolibrary.org/obo/RO_0001025 -->

    <owl:ObjectProperty rdf:about="http://purl.obolibrary.org/obo/RO_0001025"/>
    


    <!-- 
    ///////////////////////////////////////////////////////////////////////////////////////
    //
    // Classes
    //
    ///////////////////////////////////////////////////////////////////////////////////////
     -->

    


    <!-- http://purl.obolibrary.org/obo/ENVO_00000009 -->

    <owl:Class rdf:about="http://purl.obolibrary.org/obo/ENVO_00000009"/>
    


    <!-- http://purl.obolibrary.org/obo/ENVO_00000167 -->

    <owl:Class rdf:about="http://purl.obolibrary.org/obo/ENVO_00000167"/>
    


    <!-- http://purl.obolibrary.org/obo/ENVO_00000305 -->

    <owl:Class rdf:about="http://purl.obolibrary.org/obo/ENVO_00000305"/>
    


    <!-- http://purl.obolibrary.org/obo/ENVO_00000309 -->

    <owl:Class rdf:about="http://purl.obolibrary.org/obo/ENVO_00000309"/>
    


    <!-- http://purl.obolibrary.org/obo/GAZ_00009435 -->

    <owl:Class rdf:about="http://purl.obolibrary.org/obo/GAZ_00009435"/>
    


    <!-- http://purl.obolibrary.org/obo/GAZ_00014897 -->

    <owl:Class rdf:about="http://purl.obolibrary.org/obo/GAZ_00014897">
        <rdfs:subClassOf rdf:resource="http://purl.obolibrary.org/obo/GAZ_00009435"/>
    </owl:Class>
    


    <!-- http://purl.obolibrary.org/obo/GAZ_00014898 -->

    <owl:Class rdf:about="http://purl.obolibrary.org/obo/GAZ_00014898">
        <rdfs:subClassOf rdf:resource="http://purl.obolibrary.org/obo/GAZ_00009435"/>
    </owl:Class>
    


    <!-- http://purl.obolibrary.org/obo/GAZ_00014899 -->

    <owl:Class rdf:about="http://purl.obolibrary.org/obo/GAZ_00014899">
        <rdfs:subClassOf rdf:resource="http://purl.obolibrary.org/obo/GAZ_00009435"/>
    </owl:Class>
    


    <!-- http://purl.obolibrary.org/obo/GAZ_00014900 -->

    <owl:Class rdf:about="http://purl.obolibrary.org/obo/GAZ_00014900">
        <rdfs:subClassOf rdf:resource="http://purl.obolibrary.org/obo/GAZ_00009435"/>
    </owl:Class>
    


    <!-- http://purl.obolibrary.org/obo/GAZ_00014901 -->

    <owl:Class rdf:about="http://purl.obolibrary.org/obo/GAZ_00014901">
        <rdfs:subClassOf rdf:resource="http://purl.obolibrary.org/obo/GAZ_00009435"/>
    </owl:Class>
    


    <!-- http://purl.obolibrary.org/obo/GAZ_00014902 -->

    <owl:Class rdf:about="http://purl.obolibrary.org/obo/GAZ_00014902">
        <rdfs:subClassOf rdf:resource="http://purl.obolibrary.org/obo/GAZ_00009435"/>
    </owl:Class>
    


    <!-- http://purl.obolibrary.org/obo/GAZ_00014903 -->

    <owl:Class rdf:about="http://purl.obolibrary.org/obo/GAZ_00014903">
        <rdfs:subClassOf rdf:resource="http://purl.obolibrary.org/obo/GAZ_00009435"/>
    </owl:Class>
    


    <!-- http://purl.obolibrary.org/obo/GAZ_00014904 -->

    <owl:Class rdf:about="http://purl.obolibrary.org/obo/GAZ_00014904">
        <rdfs:subClassOf rdf:resource="http://purl.obolibrary.org/obo/GAZ_00009435"/>
    </owl:Class>
    


    <!-- http://purl.obolibrary.org/obo/GAZ_00014905 -->

    <owl:Class rdf:about="http://purl.obolibrary.org/obo/GAZ_00014905">
        <rdfs:subClassOf rdf:resource="http://purl.obolibrary.org/obo/GAZ_00009435"/>
    </owl:Class>
    


    <!-- http://purl.obolibrary.org/obo/GAZ_00014906 -->

    <owl:Class rdf:about="http://purl.obolibrary.org/obo/GAZ_00014906">
        <rdfs:subClassOf rdf:resource="http://purl.obolibrary.org/obo/GAZ_00009435"/>
    </owl:Class>
    


    <!-- http://purl.obolibrary.org/obo/GAZ_00014907 -->

    <owl:Class rdf:about="http://purl.obolibrary.org/obo/GAZ_00014907">
        <rdfs:subClassOf rdf:resource="http://purl.obolibrary.org/obo/GAZ_00009435"/>
    </owl:Class>
    


    <!-- http://purl.obolibrary.org/obo/GAZ_00014908 -->

    <owl:Class rdf:about="http://purl.obolibrary.org/obo/GAZ_00014908">
        <rdfs:subClassOf rdf:resource="http://purl.obolibrary.org/obo/GAZ_00009435"/>
    </owl:Class>
    


    <!-- http://purl.obolibrary.org/obo/GAZ_00014909 -->

    <owl:Class rdf:about="http://purl.obolibrary.org/obo/GAZ_00014909">
        <rdfs:subClassOf rdf:resource="http://purl.obolibrary.org/obo/GAZ_00009435"/>
        <obo:IAO_0000115>A Region of Namibia.</obo:IAO_0000115>
        <oboInOwl:hasOBONamespace>GAZ</oboInOwl:hasOBONamespace>
        <oboInOwl:id>GAZ:00014909</oboInOwl:id>
        <rdfs:label>Caprivi Region</rdfs:label>
    </owl:Class>
    


    <!-- 
    ///////////////////////////////////////////////////////////////////////////////////////
    //
    // Individuals
    //
    ///////////////////////////////////////////////////////////////////////////////////////
     -->

    


    <!-- http://purl.obolibrary.org/obo/GAZ_00001096 -->

    <owl:NamedIndividual rdf:about="http://purl.obolibrary.org/obo/GAZ_00001096">
        <rdf:type rdf:resource="http://purl.obolibrary.org/obo/ENVO_00000009"/>
        <obo:IAO_0000115>A country in southern Africa on the Atlantic coast. It shares borders with Angola and Zambia to the north, Botswana to the east, and South Africa to the south. Namibia is divided into 13 regions and subdivided into 102 constituencies.</obo:IAO_0000115>
        <oboInOwl:hasOBONamespace>GAZ</oboInOwl:hasOBONamespace>
        <oboInOwl:id>GAZ:00001096</oboInOwl:id>
        <rdfs:label>Namibia</rdfs:label>
    </owl:NamedIndividual>
    


    <!-- http://purl.obolibrary.org/obo/GAZ_00005134 -->

    <owl:NamedIndividual rdf:about="http://purl.obolibrary.org/obo/GAZ_00005134">
        <obo:RO_0001025 rdf:resource="http://purl.obolibrary.org/obo/GAZ_00044898"/>
        <obo:IAO_0000115>A waterfall on the Zambezi River.</obo:IAO_0000115>
        <oboInOwl:hasOBONamespace>GAZ</oboInOwl:hasOBONamespace>
        <oboInOwl:id>GAZ:00005134</oboInOwl:id>
        <rdfs:label>Victoria Falls</rdfs:label>
    </owl:NamedIndividual>
    


    <!-- http://purl.obolibrary.org/obo/GAZ_00007873 -->

    <owl:NamedIndividual rdf:about="http://purl.obolibrary.org/obo/GAZ_00007873">
        <obo:RO_0001025 rdf:resource="http://purl.obolibrary.org/obo/GAZ_00014906"/>
        <obo:IAO_0000115>A bay in Namibia.</obo:IAO_0000115>
        <oboInOwl:hasOBONamespace>GAZ</oboInOwl:hasOBONamespace>
        <oboInOwl:id>GAZ:00007873</oboInOwl:id>
        <rdfs:label>Walvis Bay</rdfs:label>
    </owl:NamedIndividual>
    


    <!-- http://purl.obolibrary.org/obo/GAZ_00009435 -->

    <owl:NamedIndividual rdf:about="http://purl.obolibrary.org/obo/GAZ_00009435">
        <obo:RO_0001025 rdf:resource="http://purl.obolibrary.org/obo/GAZ_00001096"/>
    </owl:NamedIndividual>
    


    <!-- http://purl.obolibrary.org/obo/GAZ_00010005 -->

    <owl:NamedIndividual rdf:about="http://purl.obolibrary.org/obo/GAZ_00010005">
        <obo:RO_0001025 rdf:resource="http://purl.obolibrary.org/obo/GAZ_00001096"/>
        <oboInOwl:hasOBONamespace>GAZ</oboInOwl:hasOBONamespace>
        <oboInOwl:id>GAZ:00010005</oboInOwl:id>
        <rdfs:label>Goas</rdfs:label>
    </owl:NamedIndividual>
    


    <!-- http://purl.obolibrary.org/obo/GAZ_00014897 -->

    <owl:NamedIndividual rdf:about="http://purl.obolibrary.org/obo/GAZ_00014897"/>
    


    <!-- http://purl.obolibrary.org/obo/GAZ_00014898 -->

    <owl:NamedIndividual rdf:about="http://purl.obolibrary.org/obo/GAZ_00014898"/>
    


    <!-- http://purl.obolibrary.org/obo/GAZ_00014899 -->

    <owl:NamedIndividual rdf:about="http://purl.obolibrary.org/obo/GAZ_00014899"/>
    


    <!-- http://purl.obolibrary.org/obo/GAZ_00014900 -->

    <owl:NamedIndividual rdf:about="http://purl.obolibrary.org/obo/GAZ_00014900"/>
    


    <!-- http://purl.obolibrary.org/obo/GAZ_00014901 -->

    <owl:NamedIndividual rdf:about="http://purl.obolibrary.org/obo/GAZ_00014901"/>
    


    <!-- http://purl.obolibrary.org/obo/GAZ_00014902 -->

    <owl:NamedIndividual rdf:about="http://purl.obolibrary.org/obo/GAZ_00014902"/>
    


    <!-- http://purl.obolibrary.org/obo/GAZ_00014903 -->

    <owl:NamedIndividual rdf:about="http://purl.obolibrary.org/obo/GAZ_00014903"/>
    


    <!-- http://purl.obolibrary.org/obo/GAZ_00014904 -->

    <owl:NamedIndividual rdf:about="http://purl.obolibrary.org/obo/GAZ_00014904"/>
    


    <!-- http://purl.obolibrary.org/obo/GAZ_00014905 -->

    <owl:NamedIndividual rdf:about="http://purl.obolibrary.org/obo/GAZ_00014905"/>
    


    <!-- http://purl.obolibrary.org/obo/GAZ_00014906 -->

    <owl:NamedIndividual rdf:about="http://purl.obolibrary.org/obo/GAZ_00014906"/>
    


    <!-- http://purl.obolibrary.org/obo/GAZ_00014907 -->

    <owl:NamedIndividual rdf:about="http://purl.obolibrary.org/obo/GAZ_00014907"/>
    


    <!-- http://purl.obolibrary.org/obo/GAZ_00014908 -->

    <owl:NamedIndividual rdf:about="http://purl.obolibrary.org/obo/GAZ_00014908"/>
    


    <!-- http://purl.obolibrary.org/obo/GAZ_00016177 -->

    <owl:NamedIndividual rdf:about="http://purl.obolibrary.org/obo/GAZ_00016177">
        <obo:IAO_0000115>A lake southwest of Harare, Zimbabwe. The lake was created and opened to the public in 1952.</obo:IAO_0000115>
        <oboInOwl:hasOBONamespace>GAZ</oboInOwl:hasOBONamespace>
        <oboInOwl:id>GAZ:00016177</oboInOwl:id>
        <rdfs:label>Lake Chivero</rdfs:label>
    </owl:NamedIndividual>
    


    <!-- http://purl.obolibrary.org/obo/GAZ_00016178 -->

    <owl:NamedIndividual rdf:about="http://purl.obolibrary.org/obo/GAZ_00016178">
        <obo:RO_0001025 rdf:resource="http://purl.obolibrary.org/obo/GAZ_00044898"/>
        <obo:IAO_0000115>A large, artificial lake and reservoir located on the Zambezi river, about halfway between the river&apos;s source and mouth, about 1300 km upstream from the Indian Ocean. The lake lies along the border between Zambia and Zimbabwe.</obo:IAO_0000115>
        <oboInOwl:hasOBONamespace>GAZ</oboInOwl:hasOBONamespace>
        <oboInOwl:id>GAZ:00016178</oboInOwl:id>
        <rdfs:label>Lake Kariba</rdfs:label>
    </owl:NamedIndividual>
    


    <!-- http://purl.obolibrary.org/obo/GAZ_00030269 -->

    <owl:NamedIndividual rdf:about="http://purl.obolibrary.org/obo/GAZ_00030269">
        <obo:IAO_0000115>An extensive national park in the Kalahari desert of Botswana. Also a subdistrict of Ghanzi District. Established 1961.</obo:IAO_0000115>
        <oboInOwl:hasOBONamespace>GAZ</oboInOwl:hasOBONamespace>
        <oboInOwl:id>GAZ:00030269</oboInOwl:id>
        <rdfs:label>Central Kalahari Game Reserve</rdfs:label>
    </owl:NamedIndividual>
    


    <!-- http://purl.obolibrary.org/obo/GAZ_00032626 -->

    <owl:NamedIndividual rdf:about="http://purl.obolibrary.org/obo/GAZ_00032626">
        <obo:IAO_0000115>A constituency in the Caprivi Region of Namibia.</obo:IAO_0000115>
        <oboInOwl:hasOBONamespace>GAZ</oboInOwl:hasOBONamespace>
        <oboInOwl:id>GAZ:00032626</oboInOwl:id>
        <rdfs:label>Katima Mulilo Urban Constituency</rdfs:label>
    </owl:NamedIndividual>
    


    <!-- http://purl.obolibrary.org/obo/GAZ_00032627 -->

    <owl:NamedIndividual rdf:about="http://purl.obolibrary.org/obo/GAZ_00032627">
        <obo:IAO_0000115>A constituency in the Caprivi Region of Namibia.</obo:IAO_0000115>
        <oboInOwl:hasOBONamespace>GAZ</oboInOwl:hasOBONamespace>
        <oboInOwl:id>GAZ:00032627</oboInOwl:id>
        <rdfs:label>Katima Mulilo Rural Constituency</rdfs:label>
    </owl:NamedIndividual>
    


    <!-- http://purl.obolibrary.org/obo/GAZ_00032628 -->

    <owl:NamedIndividual rdf:about="http://purl.obolibrary.org/obo/GAZ_00032628">
        <obo:IAO_0000115>A constituency in the Caprivi Region of Namibia.</obo:IAO_0000115>
        <oboInOwl:hasOBONamespace>GAZ</oboInOwl:hasOBONamespace>
        <oboInOwl:id>GAZ:00032628</oboInOwl:id>
        <rdfs:label>Kabbe Constituency</rdfs:label>
    </owl:NamedIndividual>
    


    <!-- http://purl.obolibrary.org/obo/GAZ_00032629 -->

    <owl:NamedIndividual rdf:about="http://purl.obolibrary.org/obo/GAZ_00032629">
        <obo:IAO_0000115>A constituency in the Caprivi Region of Namibia.</obo:IAO_0000115>
        <oboInOwl:hasOBONamespace>GAZ</oboInOwl:hasOBONamespace>
        <oboInOwl:id>GAZ:00032629</oboInOwl:id>
        <rdfs:label>Kongola Constituency</rdfs:label>
    </owl:NamedIndividual>
    


    <!-- http://purl.obolibrary.org/obo/GAZ_00032630 -->

    <owl:NamedIndividual rdf:about="http://purl.obolibrary.org/obo/GAZ_00032630">
        <obo:IAO_0000115>A constituency in the Caprivi Region of Namibia.</obo:IAO_0000115>
        <oboInOwl:hasOBONamespace>GAZ</oboInOwl:hasOBONamespace>
        <oboInOwl:id>GAZ:00032630</oboInOwl:id>
        <rdfs:label>Linyanti Constituency</rdfs:label>
    </owl:NamedIndividual>
    


    <!-- http://purl.obolibrary.org/obo/GAZ_00032631 -->

    <owl:NamedIndividual rdf:about="http://purl.obolibrary.org/obo/GAZ_00032631">
        <obo:IAO_0000115>A constituency in the Caprivi Region of Namibia.</obo:IAO_0000115>
        <oboInOwl:hasOBONamespace>GAZ</oboInOwl:hasOBONamespace>
        <oboInOwl:id>GAZ:00032631</oboInOwl:id>
        <rdfs:label>Sibinda Constituency</rdfs:label>
    </owl:NamedIndividual>
    


    <!-- http://purl.obolibrary.org/obo/GAZ_00032632 -->

    <owl:NamedIndividual rdf:about="http://purl.obolibrary.org/obo/GAZ_00032632">
        <obo:RO_0001025 rdf:resource="http://purl.obolibrary.org/obo/GAZ_00014908"/>
        <obo:IAO_0000115>A constituency in the Hardap region of Namibia.</obo:IAO_0000115>
        <oboInOwl:hasOBONamespace>GAZ</oboInOwl:hasOBONamespace>
        <oboInOwl:id>GAZ:00032632</oboInOwl:id>
        <rdfs:label>Rehoboth Rural Constituency</rdfs:label>
    </owl:NamedIndividual>
    


    <!-- http://purl.obolibrary.org/obo/GAZ_00032633 -->

    <owl:NamedIndividual rdf:about="http://purl.obolibrary.org/obo/GAZ_00032633">
        <obo:RO_0001025 rdf:resource="http://purl.obolibrary.org/obo/GAZ_00014908"/>
        <obo:IAO_0000115>A constituency in the Hardap region of Namibia.</obo:IAO_0000115>
        <oboInOwl:hasOBONamespace>GAZ</oboInOwl:hasOBONamespace>
        <oboInOwl:id>GAZ:00032633</oboInOwl:id>
        <rdfs:label>Mariental Urban Constituency</rdfs:label>
    </owl:NamedIndividual>
    


    <!-- http://purl.obolibrary.org/obo/GAZ_00032634 -->

    <owl:NamedIndividual rdf:about="http://purl.obolibrary.org/obo/GAZ_00032634">
        <obo:RO_0001025 rdf:resource="http://purl.obolibrary.org/obo/GAZ_00014908"/>
        <obo:IAO_0000115>A constituency in the Hardap region of Namibia.</obo:IAO_0000115>
        <oboInOwl:hasOBONamespace>GAZ</oboInOwl:hasOBONamespace>
        <oboInOwl:id>GAZ:00032634</oboInOwl:id>
        <rdfs:label>Gibeon Constituency</rdfs:label>
    </owl:NamedIndividual>
    


    <!-- http://purl.obolibrary.org/obo/GAZ_00032635 -->

    <owl:NamedIndividual rdf:about="http://purl.obolibrary.org/obo/GAZ_00032635">
        <obo:RO_0001025 rdf:resource="http://purl.obolibrary.org/obo/GAZ_00014906"/>
        <obo:IAO_0000115>A constituency of the Erongo Region.</obo:IAO_0000115>
        <oboInOwl:hasOBONamespace>GAZ</oboInOwl:hasOBONamespace>
        <oboInOwl:id>GAZ:00032635</oboInOwl:id>
        <rdfs:label>Swakopmund Constituency</rdfs:label>
    </owl:NamedIndividual>
    


    <!-- http://purl.obolibrary.org/obo/GAZ_00032636 -->

    <owl:NamedIndividual rdf:about="http://purl.obolibrary.org/obo/GAZ_00032636">
        <obo:RO_0001025 rdf:resource="http://purl.obolibrary.org/obo/GAZ_00014908"/>
        <obo:IAO_0000115>A constituency in the Hardap region of Namibia.</obo:IAO_0000115>
        <oboInOwl:hasOBONamespace>GAZ</oboInOwl:hasOBONamespace>
        <oboInOwl:id>GAZ:00032636</oboInOwl:id>
        <rdfs:label>Rehoboth East Urban Constituency</rdfs:label>
    </owl:NamedIndividual>
    


    <!-- http://purl.obolibrary.org/obo/GAZ_00032637 -->

    <owl:NamedIndividual rdf:about="http://purl.obolibrary.org/obo/GAZ_00032637">
        <obo:RO_0001025 rdf:resource="http://purl.obolibrary.org/obo/GAZ_00239457"/>
        <obo:IAO_0000115>A constituency in the Khomas Region of Namibia.</obo:IAO_0000115>
        <oboInOwl:hasOBONamespace>GAZ</oboInOwl:hasOBONamespace>
        <oboInOwl:id>GAZ:00032637</oboInOwl:id>
        <rdfs:label>Katutura East Constituency</rdfs:label>
    </owl:NamedIndividual>
    


    <!-- http://purl.obolibrary.org/obo/GAZ_00032638 -->

    <owl:NamedIndividual rdf:about="http://purl.obolibrary.org/obo/GAZ_00032638">
        <obo:RO_0001025 rdf:resource="http://purl.obolibrary.org/obo/GAZ_00014906"/>
        <obo:IAO_0000115>A constituency in the Erongo Region of Namibia.</obo:IAO_0000115>
        <oboInOwl:hasOBONamespace>GAZ</oboInOwl:hasOBONamespace>
        <oboInOwl:id>GAZ:00032638</oboInOwl:id>
        <rdfs:label>Arandis Constituency</rdfs:label>
    </owl:NamedIndividual>
    


    <!-- http://purl.obolibrary.org/obo/GAZ_00032639 -->

    <owl:NamedIndividual rdf:about="http://purl.obolibrary.org/obo/GAZ_00032639">
        <obo:RO_0001025 rdf:resource="http://purl.obolibrary.org/obo/GAZ_00014908"/>
        <obo:IAO_0000115>A constituency in the Hardap region of Namibia.</obo:IAO_0000115>
        <oboInOwl:hasOBONamespace>GAZ</oboInOwl:hasOBONamespace>
        <oboInOwl:id>GAZ:00032639</oboInOwl:id>
        <rdfs:label>Rehoboth West Urban Constituency</rdfs:label>
    </owl:NamedIndividual>
    


    <!-- http://purl.obolibrary.org/obo/GAZ_00032640 -->

    <owl:NamedIndividual rdf:about="http://purl.obolibrary.org/obo/GAZ_00032640">
        <obo:RO_0001025 rdf:resource="http://purl.obolibrary.org/obo/GAZ_00014906"/>
        <obo:IAO_0000115>A constituency in the Erongo Region of Namibia.</obo:IAO_0000115>
        <oboInOwl:hasOBONamespace>GAZ</oboInOwl:hasOBONamespace>
        <oboInOwl:id>GAZ:00032640</oboInOwl:id>
        <rdfs:label>Brandberg Constituency</rdfs:label>
    </owl:NamedIndividual>
    


    <!-- http://purl.obolibrary.org/obo/GAZ_00032641 -->

    <owl:NamedIndividual rdf:about="http://purl.obolibrary.org/obo/GAZ_00032641">
        <obo:RO_0001025 rdf:resource="http://purl.obolibrary.org/obo/GAZ_00014908"/>
        <obo:IAO_0000115>A constituency in the Hardap region of Namibia.</obo:IAO_0000115>
        <oboInOwl:hasOBONamespace>GAZ</oboInOwl:hasOBONamespace>
        <oboInOwl:id>GAZ:00032641</oboInOwl:id>
        <rdfs:label>Mariental Rural Constituency</rdfs:label>
    </owl:NamedIndividual>
    


    <!-- http://purl.obolibrary.org/obo/GAZ_00032642 -->

    <owl:NamedIndividual rdf:about="http://purl.obolibrary.org/obo/GAZ_00032642">
        <obo:RO_0001025 rdf:resource="http://purl.obolibrary.org/obo/GAZ_00014906"/>
        <obo:IAO_0000115>A constituency in the Erongo Region of Namibia.</obo:IAO_0000115>
        <oboInOwl:hasOBONamespace>GAZ</oboInOwl:hasOBONamespace>
        <oboInOwl:id>GAZ:00032642</oboInOwl:id>
        <rdfs:label>Omaruru Constituency</rdfs:label>
    </owl:NamedIndividual>
    


    <!-- http://purl.obolibrary.org/obo/GAZ_00032643 -->

    <owl:NamedIndividual rdf:about="http://purl.obolibrary.org/obo/GAZ_00032643">
        <obo:RO_0001025 rdf:resource="http://purl.obolibrary.org/obo/GAZ_00014906"/>
        <obo:IAO_0000115>A constituency of the Erongo Region.</obo:IAO_0000115>
        <oboInOwl:hasOBONamespace>GAZ</oboInOwl:hasOBONamespace>
        <oboInOwl:id>GAZ:00032643</oboInOwl:id>
        <rdfs:label>Walvis Bay Constituency</rdfs:label>
    </owl:NamedIndividual>
    


    <!-- http://purl.obolibrary.org/obo/GAZ_00032644 -->

    <owl:NamedIndividual rdf:about="http://purl.obolibrary.org/obo/GAZ_00032644">
        <obo:RO_0001025 rdf:resource="http://purl.obolibrary.org/obo/GAZ_00014906"/>
        <obo:IAO_0000115>A constituency in the Erongo Region of western Namibia.</obo:IAO_0000115>
        <oboInOwl:hasOBONamespace>GAZ</oboInOwl:hasOBONamespace>
        <oboInOwl:id>GAZ:00032644</oboInOwl:id>
        <rdfs:label>Karibib Constituency</rdfs:label>
    </owl:NamedIndividual>
    


    <!-- http://purl.obolibrary.org/obo/GAZ_00032645 -->

    <owl:NamedIndividual rdf:about="http://purl.obolibrary.org/obo/GAZ_00032645">
        <obo:RO_0001025 rdf:resource="http://purl.obolibrary.org/obo/GAZ_00014897"/>
        <obo:IAO_0000115>A constituency in the Kunene Region of Namibia.</obo:IAO_0000115>
        <oboInOwl:hasOBONamespace>GAZ</oboInOwl:hasOBONamespace>
        <oboInOwl:id>GAZ:00032645</oboInOwl:id>
        <rdfs:label>Outjo Constituency</rdfs:label>
    </owl:NamedIndividual>
    


    <!-- http://purl.obolibrary.org/obo/GAZ_00032646 -->

    <owl:NamedIndividual rdf:about="http://purl.obolibrary.org/obo/GAZ_00032646">
        <obo:RO_0001025 rdf:resource="http://purl.obolibrary.org/obo/GAZ_00014898"/>
        <obo:IAO_0000115>A constituency in the Khomas Region of Namibia.</obo:IAO_0000115>
        <oboInOwl:hasOBONamespace>GAZ</oboInOwl:hasOBONamespace>
        <oboInOwl:id>GAZ:00032646</oboInOwl:id>
        <rdfs:label>Windhoek Rural Constituency</rdfs:label>
    </owl:NamedIndividual>
    


    <!-- http://purl.obolibrary.org/obo/GAZ_00032647 -->

    <owl:NamedIndividual rdf:about="http://purl.obolibrary.org/obo/GAZ_00032647">
        <obo:RO_0001025 rdf:resource="http://purl.obolibrary.org/obo/GAZ_00239458"/>
        <obo:IAO_0000115>A constituency in Khomasdal, a suburb of Windhoek the Khomas Region of Namibia.</obo:IAO_0000115>
        <oboInOwl:hasOBONamespace>GAZ</oboInOwl:hasOBONamespace>
        <oboInOwl:id>GAZ:00032647</oboInOwl:id>
        <rdfs:label>Khomasdal North Constituency</rdfs:label>
    </owl:NamedIndividual>
    


    <!-- http://purl.obolibrary.org/obo/GAZ_00032648 -->

    <owl:NamedIndividual rdf:about="http://purl.obolibrary.org/obo/GAZ_00032648">
        <obo:RO_0001025 rdf:resource="http://purl.obolibrary.org/obo/GAZ_00014900"/>
        <obo:IAO_0000115>A constituency in the Karas Region of Namibia.</obo:IAO_0000115>
        <oboInOwl:hasOBONamespace>GAZ</oboInOwl:hasOBONamespace>
        <oboInOwl:id>GAZ:00032648</oboInOwl:id>
        <rdfs:label>Keetmanshoop Rural Constituency</rdfs:label>
    </owl:NamedIndividual>
    


    <!-- http://purl.obolibrary.org/obo/GAZ_00032649 -->

    <owl:NamedIndividual rdf:about="http://purl.obolibrary.org/obo/GAZ_00032649">
        <obo:RO_0001025 rdf:resource="http://purl.obolibrary.org/obo/GAZ_00014897"/>
        <obo:IAO_0000115>A constituency in Kunene Region, Namibia.</obo:IAO_0000115>
        <oboInOwl:hasOBONamespace>GAZ</oboInOwl:hasOBONamespace>
        <oboInOwl:id>GAZ:00032649</oboInOwl:id>
        <rdfs:label>Khorixas Constituency</rdfs:label>
    </owl:NamedIndividual>
    


    <!-- http://purl.obolibrary.org/obo/GAZ_00032650 -->

    <owl:NamedIndividual rdf:about="http://purl.obolibrary.org/obo/GAZ_00032650">
        <obo:RO_0001025 rdf:resource="http://purl.obolibrary.org/obo/GAZ_00239472"/>
        <obo:IAO_0000115>A constituency in the Khomas Region of Namibia. The constituency is located across the northern suburbs of Windhoek.</obo:IAO_0000115>
        <oboInOwl:hasOBONamespace>GAZ</oboInOwl:hasOBONamespace>
        <oboInOwl:id>GAZ:00032650</oboInOwl:id>
        <rdfs:label>Samora Machel Constituency</rdfs:label>
    </owl:NamedIndividual>
    


    <!-- http://purl.obolibrary.org/obo/GAZ_00032651 -->

    <owl:NamedIndividual rdf:about="http://purl.obolibrary.org/obo/GAZ_00032651">
        <obo:RO_0001025 rdf:resource="http://purl.obolibrary.org/obo/GAZ_00014900"/>
        <obo:IAO_0000115>A constituency in the Karas Region of Namibia.</obo:IAO_0000115>
        <oboInOwl:hasOBONamespace>GAZ</oboInOwl:hasOBONamespace>
        <oboInOwl:id>GAZ:00032651</oboInOwl:id>
        <rdfs:label>Keetmanshoop Urban Constituency</rdfs:label>
    </owl:NamedIndividual>
    


    <!-- http://purl.obolibrary.org/obo/GAZ_00032652 -->

    <owl:NamedIndividual rdf:about="http://purl.obolibrary.org/obo/GAZ_00032652">
        <obo:RO_0001025 rdf:resource="http://purl.obolibrary.org/obo/GAZ_00239457"/>
        <obo:IAO_0000115>A constituency in the Khomas Region of Namibia.</obo:IAO_0000115>
        <oboInOwl:hasOBONamespace>GAZ</oboInOwl:hasOBONamespace>
        <oboInOwl:id>GAZ:00032652</oboInOwl:id>
        <rdfs:label>John Pandeni Constituency</rdfs:label>
    </owl:NamedIndividual>
    


    <!-- http://purl.obolibrary.org/obo/GAZ_00032653 -->

    <owl:NamedIndividual rdf:about="http://purl.obolibrary.org/obo/GAZ_00032653">
        <obo:RO_0001025 rdf:resource="http://purl.obolibrary.org/obo/GAZ_00014900"/>
        <obo:IAO_0000115>A constituency in the Karas Region of Namibia.</obo:IAO_0000115>
        <oboInOwl:hasOBONamespace>GAZ</oboInOwl:hasOBONamespace>
        <oboInOwl:id>GAZ:00032653</oboInOwl:id>
        <rdfs:label>Karasburg Constituency</rdfs:label>
    </owl:NamedIndividual>
    


    <!-- http://purl.obolibrary.org/obo/GAZ_00032654 -->

    <owl:NamedIndividual rdf:about="http://purl.obolibrary.org/obo/GAZ_00032654">
        <obo:RO_0001025 rdf:resource="http://purl.obolibrary.org/obo/GAZ_00239457"/>
        <obo:IAO_0000115>A constituency in the Khomas Region of Namibia.</obo:IAO_0000115>
        <oboInOwl:hasOBONamespace>GAZ</oboInOwl:hasOBONamespace>
        <oboInOwl:id>GAZ:00032654</oboInOwl:id>
        <rdfs:label>Katutura Central Constituency</rdfs:label>
    </owl:NamedIndividual>
    


    <!-- http://purl.obolibrary.org/obo/GAZ_00032655 -->

    <owl:NamedIndividual rdf:about="http://purl.obolibrary.org/obo/GAZ_00032655">
        <obo:RO_0001025 rdf:resource="http://purl.obolibrary.org/obo/GAZ_00014900"/>
        <obo:IAO_0000115>A constituency in the Karas Region of Namibia.</obo:IAO_0000115>
        <oboInOwl:hasOBONamespace>GAZ</oboInOwl:hasOBONamespace>
        <oboInOwl:id>GAZ:00032655</oboInOwl:id>
        <rdfs:label>Berseba Constituency</rdfs:label>
    </owl:NamedIndividual>
    


    <!-- http://purl.obolibrary.org/obo/GAZ_00032656 -->

    <owl:NamedIndividual rdf:about="http://purl.obolibrary.org/obo/GAZ_00032656">
        <obo:RO_0001025 rdf:resource="http://purl.obolibrary.org/obo/GAZ_00239446"/>
        <obo:IAO_0000115>A constituency in the Khomas Region of Namibia.</obo:IAO_0000115>
        <oboInOwl:hasOBONamespace>GAZ</oboInOwl:hasOBONamespace>
        <oboInOwl:id>GAZ:00032656</oboInOwl:id>
        <rdfs:label>Windhoek East Constituency</rdfs:label>
    </owl:NamedIndividual>
    


    <!-- http://purl.obolibrary.org/obo/GAZ_00032657 -->

    <owl:NamedIndividual rdf:about="http://purl.obolibrary.org/obo/GAZ_00032657">
        <obo:RO_0001025 rdf:resource="http://purl.obolibrary.org/obo/GAZ_00014900"/>
        <obo:IAO_0000115>A constituency in the Karas Region of Namibia.</obo:IAO_0000115>
        <oboInOwl:hasOBONamespace>GAZ</oboInOwl:hasOBONamespace>
        <oboInOwl:id>GAZ:00032657</oboInOwl:id>
        <rdfs:label>Oranjemund Constituency</rdfs:label>
    </owl:NamedIndividual>
    


    <!-- http://purl.obolibrary.org/obo/GAZ_00032658 -->

    <owl:NamedIndividual rdf:about="http://purl.obolibrary.org/obo/GAZ_00032658">
        <obo:RO_0001025 rdf:resource="http://purl.obolibrary.org/obo/GAZ_00014900"/>
        <obo:IAO_0000115>A constituency in the Karas Region of Namibia.</obo:IAO_0000115>
        <oboInOwl:hasOBONamespace>GAZ</oboInOwl:hasOBONamespace>
        <oboInOwl:id>GAZ:00032658</oboInOwl:id>
        <rdfs:label>Luderitz Constituency</rdfs:label>
    </owl:NamedIndividual>
    


    <!-- http://purl.obolibrary.org/obo/GAZ_00032660 -->

    <owl:NamedIndividual rdf:about="http://purl.obolibrary.org/obo/GAZ_00032660">
        <obo:RO_0001025 rdf:resource="http://purl.obolibrary.org/obo/GAZ_00239446"/>
        <obo:IAO_0000115>A constituency in the Khomas Region of Namibia.</obo:IAO_0000115>
        <oboInOwl:hasOBONamespace>GAZ</oboInOwl:hasOBONamespace>
        <oboInOwl:id>GAZ:00032660</oboInOwl:id>
        <rdfs:label>Windhoek West Constituency</rdfs:label>
    </owl:NamedIndividual>
    


    <!-- http://purl.obolibrary.org/obo/GAZ_00032661 -->

    <owl:NamedIndividual rdf:about="http://purl.obolibrary.org/obo/GAZ_00032661">
        <obo:RO_0001025 rdf:resource="http://purl.obolibrary.org/obo/GAZ_00014902"/>
        <obo:IAO_0000115>A constituency of the Okavango Region.</obo:IAO_0000115>
        <oboInOwl:hasOBONamespace>GAZ</oboInOwl:hasOBONamespace>
        <oboInOwl:id>GAZ:00032661</oboInOwl:id>
        <rdfs:label>Kapako Constituency</rdfs:label>
    </owl:NamedIndividual>
    


    <!-- http://purl.obolibrary.org/obo/GAZ_00032662 -->

    <owl:NamedIndividual rdf:about="http://purl.obolibrary.org/obo/GAZ_00032662">
        <obo:RO_0001025 rdf:resource="http://purl.obolibrary.org/obo/GAZ_00014902"/>
        <obo:IAO_0000115>A constituency of the Okavango Region.</obo:IAO_0000115>
        <oboInOwl:hasOBONamespace>GAZ</oboInOwl:hasOBONamespace>
        <oboInOwl:id>GAZ:00032662</oboInOwl:id>
        <rdfs:label>Mpungu Constituency</rdfs:label>
    </owl:NamedIndividual>
    


    <!-- http://purl.obolibrary.org/obo/GAZ_00032663 -->

    <owl:NamedIndividual rdf:about="http://purl.obolibrary.org/obo/GAZ_00032663">
        <obo:RO_0001025 rdf:resource="http://purl.obolibrary.org/obo/GAZ_00014902"/>
        <obo:IAO_0000115>A constituency of the Okavango Region.</obo:IAO_0000115>
        <oboInOwl:hasOBONamespace>GAZ</oboInOwl:hasOBONamespace>
        <oboInOwl:id>GAZ:00032663</oboInOwl:id>
        <rdfs:label>Ndiyona Constituency</rdfs:label>
    </owl:NamedIndividual>
    


    <!-- http://purl.obolibrary.org/obo/GAZ_00032664 -->

    <owl:NamedIndividual rdf:about="http://purl.obolibrary.org/obo/GAZ_00032664">
        <obo:RO_0001025 rdf:resource="http://purl.obolibrary.org/obo/GAZ_00014902"/>
        <obo:IAO_0000115>A constituency of the Okavango Region.</obo:IAO_0000115>
        <oboInOwl:hasOBONamespace>GAZ</oboInOwl:hasOBONamespace>
        <oboInOwl:id>GAZ:00032664</oboInOwl:id>
        <rdfs:label>Rundu Constituency</rdfs:label>
    </owl:NamedIndividual>
    


    <!-- http://purl.obolibrary.org/obo/GAZ_00032665 -->

    <owl:NamedIndividual rdf:about="http://purl.obolibrary.org/obo/GAZ_00032665">
        <obo:RO_0001025 rdf:resource="http://purl.obolibrary.org/obo/GAZ_00014902"/>
        <obo:IAO_0000115>A constituency of the Okavango Region.</obo:IAO_0000115>
        <oboInOwl:hasOBONamespace>GAZ</oboInOwl:hasOBONamespace>
        <oboInOwl:id>GAZ:00032665</oboInOwl:id>
        <rdfs:label>Kahenge Constituency</rdfs:label>
    </owl:NamedIndividual>
    


    <!-- http://purl.obolibrary.org/obo/GAZ_00032666 -->

    <owl:NamedIndividual rdf:about="http://purl.obolibrary.org/obo/GAZ_00032666">
        <obo:RO_0001025 rdf:resource="http://purl.obolibrary.org/obo/GAZ_00014902"/>
        <obo:IAO_0000115>A constituency of the Okavango Region.</obo:IAO_0000115>
        <oboInOwl:hasOBONamespace>GAZ</oboInOwl:hasOBONamespace>
        <oboInOwl:id>GAZ:00032666</oboInOwl:id>
        <rdfs:label>Mashari Constituency</rdfs:label>
    </owl:NamedIndividual>
    


    <!-- http://purl.obolibrary.org/obo/GAZ_00032667 -->

    <owl:NamedIndividual rdf:about="http://purl.obolibrary.org/obo/GAZ_00032667">
        <obo:RO_0001025 rdf:resource="http://purl.obolibrary.org/obo/GAZ_00014897"/>
        <obo:IAO_0000115>A constituency in Kunene Region, Namibia.</obo:IAO_0000115>
        <oboInOwl:hasOBONamespace>GAZ</oboInOwl:hasOBONamespace>
        <oboInOwl:id>GAZ:00032667</oboInOwl:id>
        <rdfs:label>Sesfontein Constituency</rdfs:label>
    </owl:NamedIndividual>
    


    <!-- http://purl.obolibrary.org/obo/GAZ_00032668 -->

    <owl:NamedIndividual rdf:about="http://purl.obolibrary.org/obo/GAZ_00032668">
        <obo:RO_0001025 rdf:resource="http://purl.obolibrary.org/obo/GAZ_00014897"/>
        <obo:IAO_0000115>A constituency in the Kunene Region of Namibia.</obo:IAO_0000115>
        <oboInOwl:hasOBONamespace>GAZ</oboInOwl:hasOBONamespace>
        <oboInOwl:id>GAZ:00032668</oboInOwl:id>
        <rdfs:label>Epupa Constituency</rdfs:label>
    </owl:NamedIndividual>
    


    <!-- http://purl.obolibrary.org/obo/GAZ_00032669 -->

    <owl:NamedIndividual rdf:about="http://purl.obolibrary.org/obo/GAZ_00032669">
        <obo:RO_0001025 rdf:resource="http://purl.obolibrary.org/obo/GAZ_00014897"/>
        <obo:IAO_0000115>A constituency in the Kunene Region of Namibia.</obo:IAO_0000115>
        <oboInOwl:hasOBONamespace>GAZ</oboInOwl:hasOBONamespace>
        <oboInOwl:id>GAZ:00032669</oboInOwl:id>
        <rdfs:label>Kamanjab Constituency</rdfs:label>
    </owl:NamedIndividual>
    


    <!-- http://purl.obolibrary.org/obo/GAZ_00032670 -->

    <owl:NamedIndividual rdf:about="http://purl.obolibrary.org/obo/GAZ_00032670">
        <obo:RO_0001025 rdf:resource="http://purl.obolibrary.org/obo/GAZ_00014897"/>
        <obo:IAO_0000115>A constituency in the Kunene Region of Namibia.</obo:IAO_0000115>
        <oboInOwl:hasOBONamespace>GAZ</oboInOwl:hasOBONamespace>
        <oboInOwl:id>GAZ:00032670</oboInOwl:id>
        <rdfs:label>Opuwo Constituency</rdfs:label>
    </owl:NamedIndividual>
    


    <!-- http://purl.obolibrary.org/obo/GAZ_00032671 -->

    <owl:NamedIndividual rdf:about="http://purl.obolibrary.org/obo/GAZ_00032671">
        <obo:RO_0001025 rdf:resource="http://purl.obolibrary.org/obo/GAZ_00014905"/>
        <obo:IAO_0000115>A constituency of Ohangwena Region.</obo:IAO_0000115>
        <oboInOwl:hasOBONamespace>GAZ</oboInOwl:hasOBONamespace>
        <oboInOwl:id>GAZ:00032671</oboInOwl:id>
        <rdfs:label>OndobeConstituency</rdfs:label>
    </owl:NamedIndividual>
    


    <!-- http://purl.obolibrary.org/obo/GAZ_00032672 -->

    <owl:NamedIndividual rdf:about="http://purl.obolibrary.org/obo/GAZ_00032672">
        <obo:RO_0001025 rdf:resource="http://purl.obolibrary.org/obo/GAZ_00014905"/>
        <obo:IAO_0000115>A constituency of Ohangwena Region.</obo:IAO_0000115>
        <oboInOwl:hasOBONamespace>GAZ</oboInOwl:hasOBONamespace>
        <oboInOwl:id>GAZ:00032672</oboInOwl:id>
        <rdfs:label>Okongo Constituency</rdfs:label>
    </owl:NamedIndividual>
    


    <!-- http://purl.obolibrary.org/obo/GAZ_00032673 -->

    <owl:NamedIndividual rdf:about="http://purl.obolibrary.org/obo/GAZ_00032673">
        <obo:RO_0001025 rdf:resource="http://purl.obolibrary.org/obo/GAZ_00014905"/>
        <obo:IAO_0000115>A constituency of Ohangwena Region.</obo:IAO_0000115>
        <oboInOwl:hasOBONamespace>GAZ</oboInOwl:hasOBONamespace>
        <oboInOwl:id>GAZ:00032673</oboInOwl:id>
        <rdfs:label>Oshikango Constituency</rdfs:label>
    </owl:NamedIndividual>
    


    <!-- http://purl.obolibrary.org/obo/GAZ_00032674 -->

    <owl:NamedIndividual rdf:about="http://purl.obolibrary.org/obo/GAZ_00032674">
        <obo:RO_0001025 rdf:resource="http://purl.obolibrary.org/obo/GAZ_00014905"/>
        <obo:IAO_0000115>A constituency of Ohangwena Region.</obo:IAO_0000115>
        <oboInOwl:hasOBONamespace>GAZ</oboInOwl:hasOBONamespace>
        <oboInOwl:id>GAZ:00032674</oboInOwl:id>
        <rdfs:label>Ohangwena Constituency</rdfs:label>
    </owl:NamedIndividual>
    


    <!-- http://purl.obolibrary.org/obo/GAZ_00032675 -->

    <owl:NamedIndividual rdf:about="http://purl.obolibrary.org/obo/GAZ_00032675">
        <obo:RO_0001025 rdf:resource="http://purl.obolibrary.org/obo/GAZ_00014905"/>
        <obo:IAO_0000115>A constituency of Ohangwena Region.</obo:IAO_0000115>
        <oboInOwl:hasOBONamespace>GAZ</oboInOwl:hasOBONamespace>
        <oboInOwl:id>GAZ:00032675</oboInOwl:id>
        <rdfs:label>Engela Constituency</rdfs:label>
    </owl:NamedIndividual>
    


    <!-- http://purl.obolibrary.org/obo/GAZ_00032676 -->

    <owl:NamedIndividual rdf:about="http://purl.obolibrary.org/obo/GAZ_00032676">
        <obo:RO_0001025 rdf:resource="http://purl.obolibrary.org/obo/GAZ_00014905"/>
        <obo:IAO_0000115>A constituency of Ohangwena Region.</obo:IAO_0000115>
        <oboInOwl:hasOBONamespace>GAZ</oboInOwl:hasOBONamespace>
        <oboInOwl:id>GAZ:00032676</oboInOwl:id>
        <rdfs:label>Epembe Constituency</rdfs:label>
    </owl:NamedIndividual>
    


    <!-- http://purl.obolibrary.org/obo/GAZ_00032677 -->

    <owl:NamedIndividual rdf:about="http://purl.obolibrary.org/obo/GAZ_00032677">
        <obo:RO_0001025 rdf:resource="http://purl.obolibrary.org/obo/GAZ_00014899"/>
        <obo:IAO_0000115>A constituency in Omaheke Region, Namibia.</obo:IAO_0000115>
        <oboInOwl:hasOBONamespace>GAZ</oboInOwl:hasOBONamespace>
        <oboInOwl:id>GAZ:00032677</oboInOwl:id>
        <rdfs:label>Buitepos Constituency</rdfs:label>
    </owl:NamedIndividual>
    


    <!-- http://purl.obolibrary.org/obo/GAZ_00032678 -->

    <owl:NamedIndividual rdf:about="http://purl.obolibrary.org/obo/GAZ_00032678">
        <obo:RO_0001025 rdf:resource="http://purl.obolibrary.org/obo/GAZ_00014899"/>
        <obo:IAO_0000115>A constituency in Omaheke Region, Namibia.</obo:IAO_0000115>
        <oboInOwl:hasOBONamespace>GAZ</oboInOwl:hasOBONamespace>
        <oboInOwl:id>GAZ:00032678</oboInOwl:id>
        <rdfs:label>Gobabis Constituency</rdfs:label>
    </owl:NamedIndividual>
    


    <!-- http://purl.obolibrary.org/obo/GAZ_00032679 -->

    <owl:NamedIndividual rdf:about="http://purl.obolibrary.org/obo/GAZ_00032679">
        <obo:RO_0001025 rdf:resource="http://purl.obolibrary.org/obo/GAZ_00014899"/>
        <obo:IAO_0000115>A constituency in Omaheke Region, Namibia.</obo:IAO_0000115>
        <oboInOwl:hasOBONamespace>GAZ</oboInOwl:hasOBONamespace>
        <oboInOwl:id>GAZ:00032679</oboInOwl:id>
        <rdfs:label>Otjozondjou Constituency</rdfs:label>
    </owl:NamedIndividual>
    


    <!-- http://purl.obolibrary.org/obo/GAZ_00032680 -->

    <owl:NamedIndividual rdf:about="http://purl.obolibrary.org/obo/GAZ_00032680">
        <obo:RO_0001025 rdf:resource="http://purl.obolibrary.org/obo/GAZ_00014899"/>
        <obo:IAO_0000115>A constituency in Omaheke Region, Namibia.</obo:IAO_0000115>
        <oboInOwl:hasOBONamespace>GAZ</oboInOwl:hasOBONamespace>
        <oboInOwl:id>GAZ:00032680</oboInOwl:id>
        <rdfs:label>Otjinene Constituency</rdfs:label>
    </owl:NamedIndividual>
    


    <!-- http://purl.obolibrary.org/obo/GAZ_00032681 -->

    <owl:NamedIndividual rdf:about="http://purl.obolibrary.org/obo/GAZ_00032681">
        <obo:RO_0001025 rdf:resource="http://purl.obolibrary.org/obo/GAZ_00014899"/>
        <obo:IAO_0000115>A constituency in Omaheke Region, Namibia.</obo:IAO_0000115>
        <oboInOwl:hasOBONamespace>GAZ</oboInOwl:hasOBONamespace>
        <oboInOwl:id>GAZ:00032681</oboInOwl:id>
        <rdfs:label>Steinhausen Constituency</rdfs:label>
    </owl:NamedIndividual>
    


    <!-- http://purl.obolibrary.org/obo/GAZ_00032682 -->

    <owl:NamedIndividual rdf:about="http://purl.obolibrary.org/obo/GAZ_00032682">
        <obo:RO_0001025 rdf:resource="http://purl.obolibrary.org/obo/GAZ_00014899"/>
        <obo:IAO_0000115>A constituency in Omaheke Region, Namibia.</obo:IAO_0000115>
        <oboInOwl:hasOBONamespace>GAZ</oboInOwl:hasOBONamespace>
        <oboInOwl:id>GAZ:00032682</oboInOwl:id>
        <rdfs:label>Aminuis Constituency</rdfs:label>
    </owl:NamedIndividual>
    


    <!-- http://purl.obolibrary.org/obo/GAZ_00032683 -->

    <owl:NamedIndividual rdf:about="http://purl.obolibrary.org/obo/GAZ_00032683">
        <obo:RO_0001025 rdf:resource="http://purl.obolibrary.org/obo/GAZ_00014905"/>
        <obo:IAO_0000115>A constituency of Ohangwena Region.</obo:IAO_0000115>
        <oboInOwl:hasOBONamespace>GAZ</oboInOwl:hasOBONamespace>
        <oboInOwl:id>GAZ:00032683</oboInOwl:id>
        <rdfs:label>Endola Constituency</rdfs:label>
    </owl:NamedIndividual>
    


    <!-- http://purl.obolibrary.org/obo/GAZ_00032684 -->

    <owl:NamedIndividual rdf:about="http://purl.obolibrary.org/obo/GAZ_00032684">
        <obo:RO_0001025 rdf:resource="http://purl.obolibrary.org/obo/GAZ_00014905"/>
        <obo:IAO_0000115>A constituency of Ohangwena Region.</obo:IAO_0000115>
        <oboInOwl:hasOBONamespace>GAZ</oboInOwl:hasOBONamespace>
        <oboInOwl:id>GAZ:00032684</oboInOwl:id>
        <rdfs:label>Eenhana Constituency</rdfs:label>
    </owl:NamedIndividual>
    


    <!-- http://purl.obolibrary.org/obo/GAZ_00032685 -->

    <owl:NamedIndividual rdf:about="http://purl.obolibrary.org/obo/GAZ_00032685">
        <obo:RO_0001025 rdf:resource="http://purl.obolibrary.org/obo/GAZ_00014905"/>
        <obo:IAO_0000115>A constituency of Ohangwena Region.</obo:IAO_0000115>
        <oboInOwl:hasOBONamespace>GAZ</oboInOwl:hasOBONamespace>
        <oboInOwl:id>GAZ:00032685</oboInOwl:id>
        <rdfs:label>Omundaungilo Constituency</rdfs:label>
    </owl:NamedIndividual>
    


    <!-- http://purl.obolibrary.org/obo/GAZ_00032686 -->

    <owl:NamedIndividual rdf:about="http://purl.obolibrary.org/obo/GAZ_00032686">
        <obo:RO_0001025 rdf:resource="http://purl.obolibrary.org/obo/GAZ_00014905"/>
        <obo:IAO_0000115>A constituency of Ohangwena Region.</obo:IAO_0000115>
        <oboInOwl:hasOBONamespace>GAZ</oboInOwl:hasOBONamespace>
        <oboInOwl:id>GAZ:00032686</oboInOwl:id>
        <rdfs:label>Ongenga Constituency</rdfs:label>
    </owl:NamedIndividual>
    


    <!-- http://purl.obolibrary.org/obo/GAZ_00032687 -->

    <owl:NamedIndividual rdf:about="http://purl.obolibrary.org/obo/GAZ_00032687">
        <obo:RO_0001025 rdf:resource="http://purl.obolibrary.org/obo/GAZ_00014904"/>
        <obo:IAO_0000115>A constituency within the Omusati region.</obo:IAO_0000115>
        <oboInOwl:hasOBONamespace>GAZ</oboInOwl:hasOBONamespace>
        <oboInOwl:id>GAZ:00032687</oboInOwl:id>
        <rdfs:label>Onesi Constituency</rdfs:label>
    </owl:NamedIndividual>
    


    <!-- http://purl.obolibrary.org/obo/GAZ_00032688 -->

    <owl:NamedIndividual rdf:about="http://purl.obolibrary.org/obo/GAZ_00032688">
        <obo:RO_0001025 rdf:resource="http://purl.obolibrary.org/obo/GAZ_00014904"/>
        <obo:IAO_0000115>A constituency within the Omusati region.</obo:IAO_0000115>
        <oboInOwl:hasOBONamespace>GAZ</oboInOwl:hasOBONamespace>
        <oboInOwl:id>GAZ:00032688</oboInOwl:id>
        <rdfs:label>Oshikuku Constituency</rdfs:label>
    </owl:NamedIndividual>
    


    <!-- http://purl.obolibrary.org/obo/GAZ_00032689 -->

    <owl:NamedIndividual rdf:about="http://purl.obolibrary.org/obo/GAZ_00032689">
        <obo:RO_0001025 rdf:resource="http://purl.obolibrary.org/obo/GAZ_00014904"/>
        <obo:IAO_0000115>A constituency within the Omusati region.</obo:IAO_0000115>
        <oboInOwl:hasOBONamespace>GAZ</oboInOwl:hasOBONamespace>
        <oboInOwl:id>GAZ:00032689</oboInOwl:id>
        <rdfs:label>Elim Constituency</rdfs:label>
    </owl:NamedIndividual>
    


    <!-- http://purl.obolibrary.org/obo/GAZ_00032690 -->

    <owl:NamedIndividual rdf:about="http://purl.obolibrary.org/obo/GAZ_00032690">
        <obo:RO_0001025 rdf:resource="http://purl.obolibrary.org/obo/GAZ_00014904"/>
        <obo:IAO_0000115>A constituency within the Omusati region.</obo:IAO_0000115>
        <oboInOwl:hasOBONamespace>GAZ</oboInOwl:hasOBONamespace>
        <oboInOwl:id>GAZ:00032690</oboInOwl:id>
        <rdfs:label>Okalongo Constituency</rdfs:label>
    </owl:NamedIndividual>
    


    <!-- http://purl.obolibrary.org/obo/GAZ_00032691 -->

    <owl:NamedIndividual rdf:about="http://purl.obolibrary.org/obo/GAZ_00032691">
        <obo:RO_0001025 rdf:resource="http://purl.obolibrary.org/obo/GAZ_00014904"/>
        <obo:IAO_0000115>A constituency within the Omusati region.</obo:IAO_0000115>
        <oboInOwl:hasOBONamespace>GAZ</oboInOwl:hasOBONamespace>
        <oboInOwl:id>GAZ:00032691</oboInOwl:id>
        <rdfs:label>Anamulenge Constituency</rdfs:label>
    </owl:NamedIndividual>
    


    <!-- http://purl.obolibrary.org/obo/GAZ_00032692 -->

    <owl:NamedIndividual rdf:about="http://purl.obolibrary.org/obo/GAZ_00032692">
        <obo:RO_0001025 rdf:resource="http://purl.obolibrary.org/obo/GAZ_00014904"/>
        <obo:IAO_0000115>A constituency within the Omusati region.</obo:IAO_0000115>
        <oboInOwl:hasOBONamespace>GAZ</oboInOwl:hasOBONamespace>
        <oboInOwl:id>GAZ:00032692</oboInOwl:id>
        <rdfs:label>Okahao Constituency</rdfs:label>
    </owl:NamedIndividual>
    


    <!-- http://purl.obolibrary.org/obo/GAZ_00032693 -->

    <owl:NamedIndividual rdf:about="http://purl.obolibrary.org/obo/GAZ_00032693">
        <obo:RO_0001025 rdf:resource="http://purl.obolibrary.org/obo/GAZ_00014904"/>
        <obo:IAO_0000115>A constituency within the Omusati region.</obo:IAO_0000115>
        <oboInOwl:hasOBONamespace>GAZ</oboInOwl:hasOBONamespace>
        <oboInOwl:id>GAZ:00032693</oboInOwl:id>
        <rdfs:label>Ogongo Constituency</rdfs:label>
    </owl:NamedIndividual>
    


    <!-- http://purl.obolibrary.org/obo/GAZ_00032694 -->

    <owl:NamedIndividual rdf:about="http://purl.obolibrary.org/obo/GAZ_00032694">
        <obo:RO_0001025 rdf:resource="http://purl.obolibrary.org/obo/GAZ_00014904"/>
        <obo:IAO_0000115>A constituency within the Omusati region.</obo:IAO_0000115>
        <oboInOwl:hasOBONamespace>GAZ</oboInOwl:hasOBONamespace>
        <oboInOwl:id>GAZ:00032694</oboInOwl:id>
        <rdfs:label>Tsandi Constituency</rdfs:label>
    </owl:NamedIndividual>
    


    <!-- http://purl.obolibrary.org/obo/GAZ_00032695 -->

    <owl:NamedIndividual rdf:about="http://purl.obolibrary.org/obo/GAZ_00032695">
        <obo:RO_0001025 rdf:resource="http://purl.obolibrary.org/obo/GAZ_00014904"/>
        <obo:IAO_0000115>A constituency within the Omusati region.</obo:IAO_0000115>
        <oboInOwl:hasOBONamespace>GAZ</oboInOwl:hasOBONamespace>
        <oboInOwl:id>GAZ:00032695</oboInOwl:id>
        <rdfs:label>Uutapi Constituency</rdfs:label>
    </owl:NamedIndividual>
    


    <!-- http://purl.obolibrary.org/obo/GAZ_00032696 -->

    <owl:NamedIndividual rdf:about="http://purl.obolibrary.org/obo/GAZ_00032696">
        <obo:RO_0001025 rdf:resource="http://purl.obolibrary.org/obo/GAZ_00014903"/>
        <obo:IAO_0000115>A constutuency of Oshana Region.</obo:IAO_0000115>
        <oboInOwl:hasOBONamespace>GAZ</oboInOwl:hasOBONamespace>
        <oboInOwl:id>GAZ:00032696</oboInOwl:id>
        <rdfs:label>Uukwiyu Constituency</rdfs:label>
    </owl:NamedIndividual>
    


    <!-- http://purl.obolibrary.org/obo/GAZ_00032697 -->

    <owl:NamedIndividual rdf:about="http://purl.obolibrary.org/obo/GAZ_00032697">
        <obo:RO_0001025 rdf:resource="http://purl.obolibrary.org/obo/GAZ_00014903"/>
        <obo:IAO_0000115>A constutuency of Oshana Region.</obo:IAO_0000115>
        <oboInOwl:hasOBONamespace>GAZ</oboInOwl:hasOBONamespace>
        <oboInOwl:id>GAZ:00032697</oboInOwl:id>
        <rdfs:label>Okatana Constituency</rdfs:label>
    </owl:NamedIndividual>
    


    <!-- http://purl.obolibrary.org/obo/GAZ_00032698 -->

    <owl:NamedIndividual rdf:about="http://purl.obolibrary.org/obo/GAZ_00032698">
        <obo:RO_0001025 rdf:resource="http://purl.obolibrary.org/obo/GAZ_00014903"/>
        <obo:IAO_0000115>A constutuency of Oshana Region.</obo:IAO_0000115>
        <oboInOwl:hasOBONamespace>GAZ</oboInOwl:hasOBONamespace>
        <oboInOwl:id>GAZ:00032698</oboInOwl:id>
        <rdfs:label>Ongwediva Constituency</rdfs:label>
    </owl:NamedIndividual>
    


    <!-- http://purl.obolibrary.org/obo/GAZ_00032699 -->

    <owl:NamedIndividual rdf:about="http://purl.obolibrary.org/obo/GAZ_00032699">
        <obo:RO_0001025 rdf:resource="http://purl.obolibrary.org/obo/GAZ_00014903"/>
        <obo:IAO_0000115>A constutuency of Oshana Region.</obo:IAO_0000115>
        <oboInOwl:hasOBONamespace>GAZ</oboInOwl:hasOBONamespace>
        <oboInOwl:id>GAZ:00032699</oboInOwl:id>
        <rdfs:label>Ondangwa Constituency</rdfs:label>
    </owl:NamedIndividual>
    


    <!-- http://purl.obolibrary.org/obo/GAZ_00032700 -->

    <owl:NamedIndividual rdf:about="http://purl.obolibrary.org/obo/GAZ_00032700">
        <obo:RO_0001025 rdf:resource="http://purl.obolibrary.org/obo/GAZ_00014903"/>
        <obo:IAO_0000115>A constutuency of Oshana Region.</obo:IAO_0000115>
        <oboInOwl:hasOBONamespace>GAZ</oboInOwl:hasOBONamespace>
        <oboInOwl:id>GAZ:00032700</oboInOwl:id>
        <rdfs:label>Oshakati Constituency</rdfs:label>
    </owl:NamedIndividual>
    


    <!-- http://purl.obolibrary.org/obo/GAZ_00032701 -->

    <owl:NamedIndividual rdf:about="http://purl.obolibrary.org/obo/GAZ_00032701">
        <obo:RO_0001025 rdf:resource="http://purl.obolibrary.org/obo/GAZ_00014903"/>
        <obo:IAO_0000115>A constutuency of Oshana Region.</obo:IAO_0000115>
        <oboInOwl:hasOBONamespace>GAZ</oboInOwl:hasOBONamespace>
        <oboInOwl:id>GAZ:00032701</oboInOwl:id>
        <rdfs:label>Okatjali Constituency</rdfs:label>
    </owl:NamedIndividual>
    


    <!-- http://purl.obolibrary.org/obo/GAZ_00032702 -->

    <owl:NamedIndividual rdf:about="http://purl.obolibrary.org/obo/GAZ_00032702">
        <obo:RO_0001025 rdf:resource="http://purl.obolibrary.org/obo/GAZ_00014903"/>
        <obo:IAO_0000115>A constutuency of Oshana Region.</obo:IAO_0000115>
        <oboInOwl:hasOBONamespace>GAZ</oboInOwl:hasOBONamespace>
        <oboInOwl:id>GAZ:00032702</oboInOwl:id>
        <rdfs:label>Okaku Constituency</rdfs:label>
    </owl:NamedIndividual>
    


    <!-- http://purl.obolibrary.org/obo/GAZ_00032703 -->

    <owl:NamedIndividual rdf:about="http://purl.obolibrary.org/obo/GAZ_00032703">
        <obo:RO_0001025 rdf:resource="http://purl.obolibrary.org/obo/GAZ_00014903"/>
        <obo:IAO_0000115>A constutuency of Oshana Region.</obo:IAO_0000115>
        <oboInOwl:hasOBONamespace>GAZ</oboInOwl:hasOBONamespace>
        <oboInOwl:id>GAZ:00032703</oboInOwl:id>
        <rdfs:label>Uuvudhiya Constituency</rdfs:label>
    </owl:NamedIndividual>
    


    <!-- http://purl.obolibrary.org/obo/GAZ_00032704 -->

    <owl:NamedIndividual rdf:about="http://purl.obolibrary.org/obo/GAZ_00032704">
        <obo:RO_0001025 rdf:resource="http://purl.obolibrary.org/obo/GAZ_00014903"/>
        <obo:IAO_0000115>A constutuency of Oshana Region.</obo:IAO_0000115>
        <oboInOwl:hasOBONamespace>GAZ</oboInOwl:hasOBONamespace>
        <oboInOwl:id>GAZ:00032704</oboInOwl:id>
        <rdfs:label>Ompundja Constituency</rdfs:label>
    </owl:NamedIndividual>
    


    <!-- http://purl.obolibrary.org/obo/GAZ_00032705 -->

    <owl:NamedIndividual rdf:about="http://purl.obolibrary.org/obo/GAZ_00032705">
        <obo:RO_0001025 rdf:resource="http://purl.obolibrary.org/obo/GAZ_00014901"/>
        <obo:IAO_0000115>A constituency in Oshikoto Region, Namibia.</obo:IAO_0000115>
        <oboInOwl:hasOBONamespace>GAZ</oboInOwl:hasOBONamespace>
        <oboInOwl:id>GAZ:00032705</oboInOwl:id>
        <rdfs:label>Olukonda Constituency</rdfs:label>
    </owl:NamedIndividual>
    


    <!-- http://purl.obolibrary.org/obo/GAZ_00032706 -->

    <owl:NamedIndividual rdf:about="http://purl.obolibrary.org/obo/GAZ_00032706">
        <obo:RO_0001025 rdf:resource="http://purl.obolibrary.org/obo/GAZ_00014901"/>
        <obo:IAO_0000115>A constituency in Oshikoto Region, Namibia.</obo:IAO_0000115>
        <oboInOwl:hasOBONamespace>GAZ</oboInOwl:hasOBONamespace>
        <oboInOwl:id>GAZ:00032706</oboInOwl:id>
        <rdfs:label>Okangolo Constituency</rdfs:label>
    </owl:NamedIndividual>
    


    <!-- http://purl.obolibrary.org/obo/GAZ_00032707 -->

    <owl:NamedIndividual rdf:about="http://purl.obolibrary.org/obo/GAZ_00032707">
        <obo:RO_0001025 rdf:resource="http://purl.obolibrary.org/obo/GAZ_00014901"/>
        <obo:IAO_0000115>A constituency in Oshikoto Region, Namibia.</obo:IAO_0000115>
        <oboInOwl:hasOBONamespace>GAZ</oboInOwl:hasOBONamespace>
        <oboInOwl:id>GAZ:00032707</oboInOwl:id>
        <rdfs:label>Onayena Constituency</rdfs:label>
    </owl:NamedIndividual>
    


    <!-- http://purl.obolibrary.org/obo/GAZ_00032708 -->

    <owl:NamedIndividual rdf:about="http://purl.obolibrary.org/obo/GAZ_00032708">
        <obo:RO_0001025 rdf:resource="http://purl.obolibrary.org/obo/GAZ_00014901"/>
        <obo:IAO_0000115>A constituency in Oshikoto Region, Namibia.</obo:IAO_0000115>
        <oboInOwl:hasOBONamespace>GAZ</oboInOwl:hasOBONamespace>
        <oboInOwl:id>GAZ:00032708</oboInOwl:id>
        <rdfs:label>Omuntele Constituency</rdfs:label>
    </owl:NamedIndividual>
    


    <!-- http://purl.obolibrary.org/obo/GAZ_00032709 -->

    <owl:NamedIndividual rdf:about="http://purl.obolibrary.org/obo/GAZ_00032709">
        <obo:RO_0001025 rdf:resource="http://purl.obolibrary.org/obo/GAZ_00014901"/>
        <obo:IAO_0000115>A constituency in Oshikoto Region, Namibia.</obo:IAO_0000115>
        <oboInOwl:hasOBONamespace>GAZ</oboInOwl:hasOBONamespace>
        <oboInOwl:id>GAZ:00032709</oboInOwl:id>
        <rdfs:label>Oniipai Constituency</rdfs:label>
    </owl:NamedIndividual>
    


    <!-- http://purl.obolibrary.org/obo/GAZ_00032710 -->

    <owl:NamedIndividual rdf:about="http://purl.obolibrary.org/obo/GAZ_00032710">
        <obo:RO_0001025 rdf:resource="http://purl.obolibrary.org/obo/GAZ_00014901"/>
        <obo:IAO_0000115>A constituency in Oshikoto Region, Namibia.</obo:IAO_0000115>
        <oboInOwl:hasOBONamespace>GAZ</oboInOwl:hasOBONamespace>
        <oboInOwl:id>GAZ:00032710</oboInOwl:id>
        <rdfs:label>Engodi Constituency</rdfs:label>
    </owl:NamedIndividual>
    


    <!-- http://purl.obolibrary.org/obo/GAZ_00032711 -->

    <owl:NamedIndividual rdf:about="http://purl.obolibrary.org/obo/GAZ_00032711">
        <obo:RO_0001025 rdf:resource="http://purl.obolibrary.org/obo/GAZ_00014901"/>
        <obo:IAO_0000115>A constituency in Oshikoto Region, Namibia.</obo:IAO_0000115>
        <oboInOwl:hasOBONamespace>GAZ</oboInOwl:hasOBONamespace>
        <oboInOwl:id>GAZ:00032711</oboInOwl:id>
        <rdfs:label>Okatope Constituency</rdfs:label>
    </owl:NamedIndividual>
    


    <!-- http://purl.obolibrary.org/obo/GAZ_00032712 -->

    <owl:NamedIndividual rdf:about="http://purl.obolibrary.org/obo/GAZ_00032712">
        <obo:RO_0001025 rdf:resource="http://purl.obolibrary.org/obo/GAZ_00014901"/>
        <obo:IAO_0000115>A constituency in Oshikoto Region, Namibia.</obo:IAO_0000115>
        <oboInOwl:hasOBONamespace>GAZ</oboInOwl:hasOBONamespace>
        <oboInOwl:id>GAZ:00032712</oboInOwl:id>
        <rdfs:label>Guinas Constituency</rdfs:label>
    </owl:NamedIndividual>
    


    <!-- http://purl.obolibrary.org/obo/GAZ_00032713 -->

    <owl:NamedIndividual rdf:about="http://purl.obolibrary.org/obo/GAZ_00032713">
        <obo:RO_0001025 rdf:resource="http://purl.obolibrary.org/obo/GAZ_00014901"/>
        <obo:IAO_0000115>A constituency in Oshikoto Region, Namibia.</obo:IAO_0000115>
        <oboInOwl:hasOBONamespace>GAZ</oboInOwl:hasOBONamespace>
        <oboInOwl:id>GAZ:00032713</oboInOwl:id>
        <rdfs:label>OshikotoConstituency</rdfs:label>
    </owl:NamedIndividual>
    


    <!-- http://purl.obolibrary.org/obo/GAZ_00032714 -->

    <owl:NamedIndividual rdf:about="http://purl.obolibrary.org/obo/GAZ_00032714">
        <obo:RO_0001025 rdf:resource="http://purl.obolibrary.org/obo/GAZ_00014901"/>
        <obo:IAO_0000115>A constituency in Oshikoto Region, Namibia.</obo:IAO_0000115>
        <oboInOwl:hasOBONamespace>GAZ</oboInOwl:hasOBONamespace>
        <oboInOwl:id>GAZ:00032714</oboInOwl:id>
        <rdfs:label>Omuthiygwiipundi Constituency</rdfs:label>
    </owl:NamedIndividual>
    


    <!-- http://purl.obolibrary.org/obo/GAZ_00032715 -->

    <owl:NamedIndividual rdf:about="http://purl.obolibrary.org/obo/GAZ_00032715">
        <obo:RO_0001025 rdf:resource="http://purl.obolibrary.org/obo/GAZ_00014907"/>
        <obo:IAO_0000115>A constituency of Otjozondjupa Region.</obo:IAO_0000115>
        <oboInOwl:hasOBONamespace>GAZ</oboInOwl:hasOBONamespace>
        <oboInOwl:id>GAZ:00032715</oboInOwl:id>
        <rdfs:label>Okakarara Constituency</rdfs:label>
    </owl:NamedIndividual>
    


    <!-- http://purl.obolibrary.org/obo/GAZ_00032716 -->

    <owl:NamedIndividual rdf:about="http://purl.obolibrary.org/obo/GAZ_00032716">
        <obo:RO_0001025 rdf:resource="http://purl.obolibrary.org/obo/GAZ_00014907"/>
        <obo:IAO_0000115>A constituency of Otjozondjupa Region.</obo:IAO_0000115>
        <oboInOwl:hasOBONamespace>GAZ</oboInOwl:hasOBONamespace>
        <oboInOwl:id>GAZ:00032716</oboInOwl:id>
        <rdfs:label>Otjiwarongo Constituency</rdfs:label>
    </owl:NamedIndividual>
    


    <!-- http://purl.obolibrary.org/obo/GAZ_00032717 -->

    <owl:NamedIndividual rdf:about="http://purl.obolibrary.org/obo/GAZ_00032717">
        <obo:RO_0001025 rdf:resource="http://purl.obolibrary.org/obo/GAZ_00014907"/>
        <obo:IAO_0000115>A constituency of Otjozondjupa Region.</obo:IAO_0000115>
        <oboInOwl:hasOBONamespace>GAZ</oboInOwl:hasOBONamespace>
        <oboInOwl:id>GAZ:00032717</oboInOwl:id>
        <rdfs:label>Grootfontein Constituency</rdfs:label>
    </owl:NamedIndividual>
    


    <!-- http://purl.obolibrary.org/obo/GAZ_00032718 -->

    <owl:NamedIndividual rdf:about="http://purl.obolibrary.org/obo/GAZ_00032718">
        <obo:RO_0001025 rdf:resource="http://purl.obolibrary.org/obo/GAZ_00014907"/>
        <obo:IAO_0000115>A constituency of Otjozondjupa Region.</obo:IAO_0000115>
        <oboInOwl:hasOBONamespace>GAZ</oboInOwl:hasOBONamespace>
        <oboInOwl:id>GAZ:00032718</oboInOwl:id>
        <rdfs:label>Okahandja Constituency</rdfs:label>
    </owl:NamedIndividual>
    


    <!-- http://purl.obolibrary.org/obo/GAZ_00032719 -->

    <owl:NamedIndividual rdf:about="http://purl.obolibrary.org/obo/GAZ_00032719">
        <obo:RO_0001025 rdf:resource="http://purl.obolibrary.org/obo/GAZ_00014907"/>
        <obo:IAO_0000115>A constituency of Otjozondjupa Region.</obo:IAO_0000115>
        <oboInOwl:hasOBONamespace>GAZ</oboInOwl:hasOBONamespace>
        <oboInOwl:id>GAZ:00032719</oboInOwl:id>
        <rdfs:label>Otavi Constituency</rdfs:label>
    </owl:NamedIndividual>
    


    <!-- http://purl.obolibrary.org/obo/GAZ_00032720 -->

    <owl:NamedIndividual rdf:about="http://purl.obolibrary.org/obo/GAZ_00032720">
        <obo:RO_0001025 rdf:resource="http://purl.obolibrary.org/obo/GAZ_00014907"/>
        <obo:IAO_0000115>A constituency of Otjozondjupa Region.</obo:IAO_0000115>
        <oboInOwl:hasOBONamespace>GAZ</oboInOwl:hasOBONamespace>
        <oboInOwl:id>GAZ:00032720</oboInOwl:id>
        <rdfs:label>Omatak Constituency</rdfs:label>
    </owl:NamedIndividual>
    


    <!-- http://purl.obolibrary.org/obo/GAZ_00039982 -->

    <owl:NamedIndividual rdf:about="http://purl.obolibrary.org/obo/GAZ_00039982">
        <obo:RO_0001025 rdf:resource="http://purl.obolibrary.org/obo/GAZ_00239502"/>
        <obo:IAO_0000115>An island.</obo:IAO_0000115>
        <oboInOwl:hasOBONamespace>GAZ</oboInOwl:hasOBONamespace>
        <oboInOwl:id>GAZ:00039982</oboInOwl:id>
        <rdfs:label>Possession Island</rdfs:label>
    </owl:NamedIndividual>
    


    <!-- http://purl.obolibrary.org/obo/GAZ_00039983 -->

    <owl:NamedIndividual rdf:about="http://purl.obolibrary.org/obo/GAZ_00039983">
        <obo:RO_0001025 rdf:resource="http://purl.obolibrary.org/obo/GAZ_00239502"/>
        <obo:IAO_0000115>An island.</obo:IAO_0000115>
        <oboInOwl:hasOBONamespace>GAZ</oboInOwl:hasOBONamespace>
        <oboInOwl:id>GAZ:00039983</oboInOwl:id>
        <rdfs:label>Plumpudding Island</rdfs:label>
    </owl:NamedIndividual>
    


    <!-- http://purl.obolibrary.org/obo/GAZ_00039984 -->

    <owl:NamedIndividual rdf:about="http://purl.obolibrary.org/obo/GAZ_00039984">
        <obo:RO_0001025 rdf:resource="http://purl.obolibrary.org/obo/GAZ_00239502"/>
        <obo:IAO_0000115>An island.</obo:IAO_0000115>
        <oboInOwl:hasOBONamespace>GAZ</oboInOwl:hasOBONamespace>
        <oboInOwl:id>GAZ:00039984</oboInOwl:id>
        <rdfs:label>South Long Island</rdfs:label>
    </owl:NamedIndividual>
    


    <!-- http://purl.obolibrary.org/obo/GAZ_00039985 -->

    <owl:NamedIndividual rdf:about="http://purl.obolibrary.org/obo/GAZ_00039985">
        <obo:RO_0001025 rdf:resource="http://purl.obolibrary.org/obo/GAZ_00239502"/>
        <obo:IAO_0000115>An island.</obo:IAO_0000115>
        <oboInOwl:hasOBONamespace>GAZ</oboInOwl:hasOBONamespace>
        <oboInOwl:id>GAZ:00039985</oboInOwl:id>
        <rdfs:label>North Long Island</rdfs:label>
    </owl:NamedIndividual>
    


    <!-- http://purl.obolibrary.org/obo/GAZ_00039986 -->

    <owl:NamedIndividual rdf:about="http://purl.obolibrary.org/obo/GAZ_00039986">
        <obo:RO_0001025 rdf:resource="http://purl.obolibrary.org/obo/GAZ_00044898"/>
        <obo:IAO_0000115>An island that lies where the Chobe River flows into the Zambezi River, forming the easternmost point of Namibia. It neighbours Zambia, Botswana and Zimbabwe.</obo:IAO_0000115>
        <oboInOwl:hasOBONamespace>GAZ</oboInOwl:hasOBONamespace>
        <oboInOwl:id>GAZ:00039986</oboInOwl:id>
        <rdfs:label>Mpalila Island</rdfs:label>
    </owl:NamedIndividual>
    


    <!-- http://purl.obolibrary.org/obo/GAZ_00039987 -->

    <owl:NamedIndividual rdf:about="http://purl.obolibrary.org/obo/GAZ_00039987">
        <obo:RO_0001025 rdf:resource="http://purl.obolibrary.org/obo/GAZ_00032658"/>
        <obo:IAO_0000115>A small peninsula adjacent to the coastal city of Luderitz. Formerly an island, it became a peninsula from 1906 on by the creation of a wide land connection that doubled its former size.</obo:IAO_0000115>
        <oboInOwl:hasOBONamespace>GAZ</oboInOwl:hasOBONamespace>
        <oboInOwl:id>GAZ:00039987</oboInOwl:id>
        <rdfs:label>Shark Island</rdfs:label>
    </owl:NamedIndividual>
    


    <!-- http://purl.obolibrary.org/obo/GAZ_00039988 -->

    <owl:NamedIndividual rdf:about="http://purl.obolibrary.org/obo/GAZ_00039988">
        <obo:RO_0001025 rdf:resource="http://purl.obolibrary.org/obo/GAZ_00239502"/>
        <oboInOwl:hasOBONamespace>GAZ</oboInOwl:hasOBONamespace>
        <oboInOwl:id>GAZ:00039988</oboInOwl:id>
        <rdfs:label>False Plum Pudding Island</rdfs:label>
    </owl:NamedIndividual>
    


    <!-- http://purl.obolibrary.org/obo/GAZ_00039989 -->

    <owl:NamedIndividual rdf:about="http://purl.obolibrary.org/obo/GAZ_00039989">
        <obo:RO_0001025 rdf:resource="http://purl.obolibrary.org/obo/GAZ_00239502"/>
        <obo:IAO_0000115>An island.</obo:IAO_0000115>
        <oboInOwl:hasOBONamespace>GAZ</oboInOwl:hasOBONamespace>
        <oboInOwl:id>GAZ:00039989</oboInOwl:id>
        <rdfs:label>Pomona Island</rdfs:label>
    </owl:NamedIndividual>
    


    <!-- http://purl.obolibrary.org/obo/GAZ_00039990 -->

    <owl:NamedIndividual rdf:about="http://purl.obolibrary.org/obo/GAZ_00039990">
        <obo:RO_0001025 rdf:resource="http://purl.obolibrary.org/obo/GAZ_00032658"/>
        <obo:RO_0001025 rdf:resource="http://purl.obolibrary.org/obo/GAZ_00239502"/>
        <obo:IAO_0000115>An island N of Ludentz.</obo:IAO_0000115>
        <oboInOwl:hasOBONamespace>GAZ</oboInOwl:hasOBONamespace>
        <oboInOwl:id>GAZ:00039990</oboInOwl:id>
        <rdfs:label>Flamingo Island</rdfs:label>
    </owl:NamedIndividual>
    


    <!-- http://purl.obolibrary.org/obo/GAZ_00039991 -->

    <owl:NamedIndividual rdf:about="http://purl.obolibrary.org/obo/GAZ_00039991">
        <obo:RO_0001025 rdf:resource="http://purl.obolibrary.org/obo/GAZ_00239502"/>
        <oboInOwl:hasOBONamespace>GAZ</oboInOwl:hasOBONamespace>
        <oboInOwl:id>GAZ:00039991</oboInOwl:id>
        <rdfs:label>Seal Island</rdfs:label>
    </owl:NamedIndividual>
    


    <!-- http://purl.obolibrary.org/obo/GAZ_00039992 -->

    <owl:NamedIndividual rdf:about="http://purl.obolibrary.org/obo/GAZ_00039992">
        <obo:RO_0001025 rdf:resource="http://purl.obolibrary.org/obo/GAZ_00239502"/>
        <oboInOwl:hasOBONamespace>GAZ</oboInOwl:hasOBONamespace>
        <oboInOwl:id>GAZ:00039992</oboInOwl:id>
        <rdfs:label>Penguin Island</rdfs:label>
    </owl:NamedIndividual>
    


    <!-- http://purl.obolibrary.org/obo/GAZ_00039993 -->

    <owl:NamedIndividual rdf:about="http://purl.obolibrary.org/obo/GAZ_00039993">
        <obo:RO_0001025 rdf:resource="http://purl.obolibrary.org/obo/GAZ_00239502"/>
        <obo:IAO_0000115>An island.</obo:IAO_0000115>
        <oboInOwl:hasOBONamespace>GAZ</oboInOwl:hasOBONamespace>
        <oboInOwl:id>GAZ:00039993</oboInOwl:id>
        <rdfs:label>Sinclair&apos;s Island</rdfs:label>
    </owl:NamedIndividual>
    


    <!-- http://purl.obolibrary.org/obo/GAZ_00039994 -->

    <owl:NamedIndividual rdf:about="http://purl.obolibrary.org/obo/GAZ_00039994">
        <obo:RO_0001025 rdf:resource="http://purl.obolibrary.org/obo/GAZ_00032658"/>
        <obo:RO_0001025 rdf:resource="http://purl.obolibrary.org/obo/GAZ_00239502"/>
        <obo:IAO_0000115>An island.</obo:IAO_0000115>
        <oboInOwl:hasOBONamespace>GAZ</oboInOwl:hasOBONamespace>
        <oboInOwl:id>GAZ:00039994</oboInOwl:id>
        <rdfs:label>Halifax Island</rdfs:label>
    </owl:NamedIndividual>
    


    <!-- http://purl.obolibrary.org/obo/GAZ_00039995 -->

    <owl:NamedIndividual rdf:about="http://purl.obolibrary.org/obo/GAZ_00039995">
        <obo:RO_0001025 rdf:resource="http://purl.obolibrary.org/obo/GAZ_00239502"/>
        <obo:IAO_0000115>An island.</obo:IAO_0000115>
        <oboInOwl:hasOBONamespace>GAZ</oboInOwl:hasOBONamespace>
        <oboInOwl:id>GAZ:00039995</oboInOwl:id>
        <rdfs:label>Roastbeef Island</rdfs:label>
    </owl:NamedIndividual>
    


    <!-- http://purl.obolibrary.org/obo/GAZ_00039996 -->

    <owl:NamedIndividual rdf:about="http://purl.obolibrary.org/obo/GAZ_00039996">
        <obo:RO_0001025 rdf:resource="http://purl.obolibrary.org/obo/GAZ_00239499"/>
        <obo:RO_0001025 rdf:resource="http://purl.obolibrary.org/obo/GAZ_00239502"/>
        <obo:IAO_0000115>A small rocky island off The Diamond Coast, Namibia.</obo:IAO_0000115>
        <oboInOwl:hasOBONamespace>GAZ</oboInOwl:hasOBONamespace>
        <oboInOwl:id>GAZ:00039996</oboInOwl:id>
        <rdfs:label>Mercury Island</rdfs:label>
    </owl:NamedIndividual>
    


    <!-- http://purl.obolibrary.org/obo/GAZ_00039997 -->

    <owl:NamedIndividual rdf:about="http://purl.obolibrary.org/obo/GAZ_00039997">
        <obo:RO_0001025 rdf:resource="http://purl.obolibrary.org/obo/GAZ_00014906"/>
        <obo:IAO_0000115>A man-made platform off the coast of Namibia between Walvis Bay and Swakopmund.</obo:IAO_0000115>
        <oboInOwl:hasOBONamespace>GAZ</oboInOwl:hasOBONamespace>
        <oboInOwl:id>GAZ:00039997</oboInOwl:id>
        <rdfs:label>Bird Island</rdfs:label>
    </owl:NamedIndividual>
    


    <!-- http://purl.obolibrary.org/obo/GAZ_00039998 -->

    <owl:NamedIndividual rdf:about="http://purl.obolibrary.org/obo/GAZ_00039998">
        <obo:RO_0001025 rdf:resource="http://purl.obolibrary.org/obo/GAZ_00239502"/>
        <obo:IAO_0000115>An island.</obo:IAO_0000115>
        <oboInOwl:hasOBONamespace>GAZ</oboInOwl:hasOBONamespace>
        <oboInOwl:id>GAZ:00039998</oboInOwl:id>
        <rdfs:label>Black Rock Island</rdfs:label>
    </owl:NamedIndividual>
    


    <!-- http://purl.obolibrary.org/obo/GAZ_00039999 -->

    <owl:NamedIndividual rdf:about="http://purl.obolibrary.org/obo/GAZ_00039999">
        <obo:RO_0001025 rdf:resource="http://purl.obolibrary.org/obo/GAZ_00239502"/>
        <obo:IAO_0000115>An island.</obo:IAO_0000115>
        <oboInOwl:hasOBONamespace>GAZ</oboInOwl:hasOBONamespace>
        <oboInOwl:id>GAZ:00039999</oboInOwl:id>
        <rdfs:label>Albatross Island</rdfs:label>
    </owl:NamedIndividual>
    


    <!-- http://purl.obolibrary.org/obo/GAZ_00041529 -->

    <owl:NamedIndividual rdf:about="http://purl.obolibrary.org/obo/GAZ_00041529">
        <obo:IAO_0000115>A lake in southern part of Malawi, in the Southern Region.</obo:IAO_0000115>
        <oboInOwl:hasOBONamespace>GAZ</oboInOwl:hasOBONamespace>
        <oboInOwl:id>GAZ:00041529</oboInOwl:id>
        <rdfs:label>Lake Malombe</rdfs:label>
    </owl:NamedIndividual>
    


    <!-- http://purl.obolibrary.org/obo/GAZ_00044898 -->

    <owl:NamedIndividual rdf:about="http://purl.obolibrary.org/obo/GAZ_00044898">
        <obo:IAO_0000115>A river that rises in a black marshy dambo in north-western Zambia, in undulating miombo woodland, quite dense in parts, about 1,500 m above sea level. Eastward of the source the watershed between the Congo and Zambezi basins is a well-marked belt of high ground, falling abruptly north and south, and running nearly east-west. This distinctly cuts off the basin of the Lualaba (the main branch of the upper Congo) from that of the Zambezi. In the neighborhood of the source the watershed is not as clearly defined, but the two river systems do not connect. The river flows to the south-west and into Angola for about 240 km, then is joined by sizeable tributaries such as the Luena and the Chifumage flowing from highlands to the north-west. It turns south and develops a floodplain and becomes very variable in width between the dry and rainy seasons. It enters a region with dense patches of evergreen Cryptosepalum dry forest, though on its wesern side, Western Zambezian grasslands also occur. Where it re-enters Zambia it is nearly 400 m wide in the rainy season and flows quite quickly with rapids ending in the Chavuma Falls, where the river flows through a rocky fissure. The river drops about 400 m in elevation from its source to the at 1500 m to the Chavuma Falls at 1100 metres, in a distance of about 400 km. From this point to the Victoria Falls, the level of the basin is very uniform, dropping only by another 180 m in a distance of around 800 km. The first of its large tributaries to enter the Zambezi is the Kabompo River in the north-western province of Zambia. The savanna through which the river has flowed gives way to a wide floodplain, studded with Borassus fan palms. A little farther south is the confluence with the Lungwebungu River. This is the beginning of the Barotse Floodplain, the most notable feature of the upper Zambezi, but this northern part does not flood so much and includes islands of higher land in the middle. Thirty km below the confluence of the Lungwebungu the country becomes very flat, and the typical Barotse Floodplain landscape unfolds, with the flood reaching a width of 25 km in the rainy season. For more than 200 km downstream the annual flood cycle dominates the natural environment and human life, society and culture. Eighty km further down, the Luanginga, which with its tributaries drains a large area to the west, joins the Zambezi. A few km higher up on the east the main stream is joined in the rainy season by overflow of the Luampa/Luena system. The Victoria Falls are considered the boundary between the upper and middle Zambezi. Below them the river continues to flow due east for about 200 km, cutting through perpendicular walls of basalt 20 to 60 m apart in hills 200 to 250 m high. The river flows swiftly through the gorge, the current being continually interrupted by reefs. Beyond the gorge are a succession of rapids which end 240 km below Victoria Falls. Over this distance, the river drops 250 m. At this point, the river enters Lake Kariba, created in 1959 following the completion of the Kariba Dam. The lake is one of the largest artificial lakes in the world, and the hydroelectric power-generating facilities at the dam provide electricity to much of Zambia and Zimbabwe. The Luangwa and the Kafue are the two largest left-hand tributaries of the Zambezi. The Kafue joins the main river in a quiet deep stream about 180 m wide. From this point the northward bend of the Zambezi is checked and the stream continues due east. At the confluence of the Luangwa it enters Mozambique. The middle Zambezi ends when the river enters Lake Cahora Bassa (also spelled Cabora Bassa). Formerly the site of dangerous rapids known as Kebrabassa, the lake was created in 1974 by the construction of the Cahora Bassa Dam. The lower Zambezi&apos;s 650 km from Cahora Bassa to the Indian Ocean is navigable, although the river is shallow in many places during the dry season. This shallowness arises as the river enters a broad valley and spreads out over a large area. Only at one point, the Lupata Gorge, 320 km from its mouth, is the river confined between high hills. Here it is scarcely 200 m wide. Elsewhere it is from 5 to 8 km wide, flowing gently in many streams. The river bed is sandy, and the banks are low and reed-fringed. At places, however, and especially in the rainy season, the streams unite into one broad fast-flowing river. About 160 km from the sea the Zambezi receives the drainage of Lake Malawi through the Shire River. On approaching the Indian Ocean, the river splits up into a number of branches and forms a wide delta. Each of the four principal mouths, Milambe, Kongone, Luabo and Timbwe, is obstructed by a sand bar. A more northerly branch, called the Chinde mouth, has a minimum depth at low water of 2 m at the entrance and 4 m further in, and is the branch used for navigation. 100 km further north is a river called the Quelimane, after the town at its mouth. This stream, which is silting up, receives the overflow of the Zambezi in the rainy season. The delta of the Zambezi is today about half as broad as it was before the construction of the Kariba and Cahora Bassa dams controlled the seasonal variations in the flow rate of the river. A short distance downstream of the confluence with the Luanginga is Lealui, after which, the river turns to south-south-east. From the east it continues to receive numerous small streams, but on the west is without major tributaries for 240 km. Before this, the Ngonye Falls and subsequent rapids interrupt navigation. South of Ngonye Falls, the river briefly borders Namibia&apos;s Caprivi Strip. The strip projects from the main body of Namibia, and results from the colonial era: it was added to German South-West Africa expressly to give Germany access to the Zambezi. Below the junction of the Cuando River and the Zambezi the river bends almost due east. Here, the river is very broad and shallow, and flows fairly slowly, but as it flows eastward towards the border of the great central plateau of Africa it reaches a chasm into which the Victoria Falls plunge.</obo:IAO_0000115>
        <oboInOwl:hasOBONamespace>GAZ</oboInOwl:hasOBONamespace>
        <oboInOwl:id>GAZ:00044898</oboInOwl:id>
        <rdfs:label>Zambezi River</rdfs:label>
    </owl:NamedIndividual>
    


    <!-- http://purl.obolibrary.org/obo/GAZ_00044899 -->

    <owl:NamedIndividual rdf:about="http://purl.obolibrary.org/obo/GAZ_00044899">
        <obo:RO_0001025 rdf:resource="http://purl.obolibrary.org/obo/GAZ_00016178"/>
        <obo:IAO_0000115>An island of Lake Kariba.</obo:IAO_0000115>
        <oboInOwl:hasOBONamespace>GAZ</oboInOwl:hasOBONamespace>
        <oboInOwl:id>GAZ:00044899</oboInOwl:id>
        <rdfs:label>Chete Island</rdfs:label>
    </owl:NamedIndividual>
    


    <!-- http://purl.obolibrary.org/obo/GAZ_00044900 -->

    <owl:NamedIndividual rdf:about="http://purl.obolibrary.org/obo/GAZ_00044900">
        <obo:RO_0001025 rdf:resource="http://purl.obolibrary.org/obo/GAZ_00016178"/>
        <obo:IAO_0000115>An island of Lake Kariba.</obo:IAO_0000115>
        <oboInOwl:hasOBONamespace>GAZ</oboInOwl:hasOBONamespace>
        <oboInOwl:id>GAZ:00044900</oboInOwl:id>
        <rdfs:label>Sekula Island</rdfs:label>
    </owl:NamedIndividual>
    


    <!-- http://purl.obolibrary.org/obo/GAZ_00044901 -->

    <owl:NamedIndividual rdf:about="http://purl.obolibrary.org/obo/GAZ_00044901">
        <obo:RO_0001025 rdf:resource="http://purl.obolibrary.org/obo/GAZ_00016178"/>
        <obo:IAO_0000115>An island of Lake Kariba.</obo:IAO_0000115>
        <oboInOwl:hasOBONamespace>GAZ</oboInOwl:hasOBONamespace>
        <oboInOwl:id>GAZ:00044901</oboInOwl:id>
        <rdfs:label>Chikanka Island</rdfs:label>
    </owl:NamedIndividual>
    


    <!-- http://purl.obolibrary.org/obo/GAZ_00044913 -->

    <owl:NamedIndividual rdf:about="http://purl.obolibrary.org/obo/GAZ_00044913">
        <obo:RO_0001025 rdf:resource="http://purl.obolibrary.org/obo/GAZ_00044898"/>
        <obo:IAO_0000115>An artificial lake, being an impoundment of the middle Zambezi River. Constructed 1966-1975.</obo:IAO_0000115>
        <oboInOwl:hasOBONamespace>GAZ</oboInOwl:hasOBONamespace>
        <oboInOwl:id>GAZ:00044913</oboInOwl:id>
        <rdfs:label>Cahora Bassa</rdfs:label>
    </owl:NamedIndividual>
    


    <!-- http://purl.obolibrary.org/obo/GAZ_00051195 -->

    <owl:NamedIndividual rdf:about="http://purl.obolibrary.org/obo/GAZ_00051195">
        <obo:IAO_0000115>A large endorheic salt pan, forming part of the Kalahari Basin in the north of Namibia. The sole source of water is the Ekuma River.</obo:IAO_0000115>
        <oboInOwl:hasOBONamespace>GAZ</oboInOwl:hasOBONamespace>
        <oboInOwl:id>GAZ:00051195</oboInOwl:id>
        <rdfs:label>Etosha Pan</rdfs:label>
    </owl:NamedIndividual>
    


    <!-- http://purl.obolibrary.org/obo/GAZ_00052629 -->

    <owl:NamedIndividual rdf:about="http://purl.obolibrary.org/obo/GAZ_00052629">
        <obo:IAO_0000115>A river that is a major tributary of the Zambezi River. The Luwangwa rises in the Lilonda and Mafinga Hills in north-east Zambia at an elevation of around 1500 m, near the border with Tanzania and Malawi, and flows in a southwesterly direction through a broad valley. About 150 km from its source it has dropped to an elevation of about 690 m and becomes a meandering river with a flood-plain several km wide. Over the next 300 km the meanders increase, with many ox-bow lakes and abandoned meanders. Near Mfuwe, the river&apos;s elevation has dropped to about 520 m, the flood plain is about 10 km wide and the valley reaches about 100 km wide, with a north-west escarpment (Muchinga Escarpment) about 700 m high, and a south-western escarpment about 450 m high. In the dry season some sections, especially in the upper reaches, dry out completely, leaving isolated pools. At about 500 km the valley narrows to about 50 km and becomes divided by a ridge into two parallel valleys, with a tributary, the Lukusashi River in a 25 km-wide valley to the north-west, and the Luangwa in a 15 km wide valley to the southeast. The river meanders less, and the flood plain narrows. At 600 km the river abruptly enters a narrow valley between hills rising some 200 m from the broader valley floor, becoming almost a gorge. About 700 km from source the Luangwa merges with its tributary the Lukusashi after the latter has merged with the Lunsemfwa River coming from the oppostie driection, and turns due south through a steep narrow valley: this is its exit from the Luangwa Rift Valley (see following section). After only 20 km it emerges from the hills into the broad valley of the Zambezi and meanders over sandy flats about 1.5 km wide in a flood plain of 3-5 km wide. It merges with the deeper Zambezi at Luangwa town.</obo:IAO_0000115>
        <oboInOwl:hasOBONamespace>GAZ</oboInOwl:hasOBONamespace>
        <oboInOwl:id>GAZ:00052629</oboInOwl:id>
        <rdfs:label>Luangwa River</rdfs:label>
    </owl:NamedIndividual>
    


    <!-- http://purl.obolibrary.org/obo/GAZ_00052649 -->

    <owl:NamedIndividual rdf:about="http://purl.obolibrary.org/obo/GAZ_00052649">
        <obo:IAO_0000115>A dam on the Kafue River in west-central Zambia at the Itezhi-Tezhi Gap, in a range of hills through which the river had eroded a narrow valley, leading to the broad expanse of the wetlands known as the Kafue Flats. Constructed 1974-1977.</obo:IAO_0000115>
        <oboInOwl:hasOBONamespace>GAZ</oboInOwl:hasOBONamespace>
        <oboInOwl:id>GAZ:00052649</oboInOwl:id>
        <rdfs:label>Itezhi-Tezhi Dam</rdfs:label>
    </owl:NamedIndividual>
    


    <!-- http://purl.obolibrary.org/obo/GAZ_00057764 -->

    <owl:NamedIndividual rdf:about="http://purl.obolibrary.org/obo/GAZ_00057764">
        <obo:RO_0001025 rdf:resource="http://purl.obolibrary.org/obo/GAZ_00014900"/>
        <obo:IAO_0000115>The N part of Namaqualand, located in the Karas Region of Namibia.</obo:IAO_0000115>
        <oboInOwl:hasOBONamespace>GAZ</oboInOwl:hasOBONamespace>
        <oboInOwl:id>GAZ:00057764</oboInOwl:id>
        <rdfs:label>Great Namaqualand</rdfs:label>
    </owl:NamedIndividual>
    


    <!-- http://purl.obolibrary.org/obo/GAZ_00058784 -->

    <owl:NamedIndividual rdf:about="http://purl.obolibrary.org/obo/GAZ_00058784">
        <obo:RO_0001025 rdf:resource="http://purl.obolibrary.org/obo/GAZ_00058785"/>
        <obo:IAO_0000115>A reservoir SE of Kabwe, Zambia due to the construction by the Broken Hill Development Company of the Mulungushi Dam on the Mulungushi River. Completed 1925.</obo:IAO_0000115>
        <oboInOwl:hasOBONamespace>GAZ</oboInOwl:hasOBONamespace>
        <oboInOwl:id>GAZ:00058784</oboInOwl:id>
        <rdfs:label>Mulungushi Lake</rdfs:label>
    </owl:NamedIndividual>
    


    <!-- http://purl.obolibrary.org/obo/GAZ_00058785 -->

    <owl:NamedIndividual rdf:about="http://purl.obolibrary.org/obo/GAZ_00058785">
        <obo:IAO_0000115>A river in central Zambia is a tributary of the Lunsemfwa River and the Luangwa River, and a part of the Zambezi River basin. It rises on the plateau north-west of Kabwe and flows south-east into the Luangwa Rift Valley where it joins the Lunsemfwa.</obo:IAO_0000115>
        <oboInOwl:hasOBONamespace>GAZ</oboInOwl:hasOBONamespace>
        <oboInOwl:id>GAZ:00058785</oboInOwl:id>
        <rdfs:label>Mulungushi River</rdfs:label>
    </owl:NamedIndividual>
    


    <!-- http://purl.obolibrary.org/obo/GAZ_00058814 -->

    <owl:NamedIndividual rdf:about="http://purl.obolibrary.org/obo/GAZ_00058814">
        <obo:IAO_0000115>A dam, constructed in 1938, on the Vaal River.</obo:IAO_0000115>
        <oboInOwl:hasOBONamespace>GAZ</oboInOwl:hasOBONamespace>
        <oboInOwl:id>GAZ:00058814</oboInOwl:id>
        <rdfs:label>Vaal Dam</rdfs:label>
    </owl:NamedIndividual>
    


    <!-- http://purl.obolibrary.org/obo/GAZ_00058815 -->

    <owl:NamedIndividual rdf:about="http://purl.obolibrary.org/obo/GAZ_00058815">
        <obo:IAO_0000115>A reservoir caused by the construction of the Vaal Dam in 1938. Three Provinces make up the coastline. The Free State is the largest by area, Mpumalanga, and Gauteng.</obo:IAO_0000115>
        <oboInOwl:hasOBONamespace>GAZ</oboInOwl:hasOBONamespace>
        <oboInOwl:id>GAZ:00058815</oboInOwl:id>
        <rdfs:label>Vaal Dam Lake</rdfs:label>
    </owl:NamedIndividual>
    


    <!-- http://purl.obolibrary.org/obo/GAZ_00075422 -->

    <owl:NamedIndividual rdf:about="http://purl.obolibrary.org/obo/GAZ_00075422">
        <obo:IAO_0000115>A large salt pan complex in Northern Botswana, the largest salt flat complex in the world. These salt pans cover 16,000 km2 and form the bed of an ancient lake that started evaporating 10,000 years ago. The main water source is the Nata River, called Amanzinyama in Zimbabwe where it rises at Sandown about 60 km from Bulawayo.</obo:IAO_0000115>
        <oboInOwl:hasOBONamespace>GAZ</oboInOwl:hasOBONamespace>
        <oboInOwl:id>GAZ:00075422</oboInOwl:id>
        <rdfs:label>Makgadikgadi Pans</rdfs:label>
    </owl:NamedIndividual>
    


    <!-- http://purl.obolibrary.org/obo/GAZ_00075423 -->

    <owl:NamedIndividual rdf:about="http://purl.obolibrary.org/obo/GAZ_00075423">
        <obo:RO_0001025 rdf:resource="http://purl.obolibrary.org/obo/GAZ_00237428"/>
        <obo:IAO_0000115>A dry granite rock island located in the Makgadikgadi Pans National Park area of Botswana.</obo:IAO_0000115>
        <oboInOwl:hasOBONamespace>GAZ</oboInOwl:hasOBONamespace>
        <oboInOwl:id>GAZ:00075423</oboInOwl:id>
        <rdfs:label>Kubu Island</rdfs:label>
    </owl:NamedIndividual>
    


    <!-- http://purl.obolibrary.org/obo/GAZ_00075424 -->

    <owl:NamedIndividual rdf:about="http://purl.obolibrary.org/obo/GAZ_00075424">
        <obo:RO_0001025 rdf:resource="http://purl.obolibrary.org/obo/GAZ_00075422"/>
        <oboInOwl:hasOBONamespace>GAZ</oboInOwl:hasOBONamespace>
        <oboInOwl:id>GAZ:00075424</oboInOwl:id>
        <rdfs:label>Makgadikgadi Pans National Park</rdfs:label>
    </owl:NamedIndividual>
    


    <!-- http://purl.obolibrary.org/obo/GAZ_00076291 -->

    <owl:NamedIndividual rdf:about="http://purl.obolibrary.org/obo/GAZ_00076291">
        <obo:RO_0001025 rdf:resource="http://purl.obolibrary.org/obo/GAZ_00075422"/>
        <obo:IAO_0000115>A national park in Botswana.</obo:IAO_0000115>
        <oboInOwl:hasOBONamespace>GAZ</oboInOwl:hasOBONamespace>
        <oboInOwl:id>GAZ:00076291</oboInOwl:id>
        <rdfs:label>Nxai Pan National Park</rdfs:label>
    </owl:NamedIndividual>
    


    <!-- http://purl.obolibrary.org/obo/GAZ_00076293 -->

    <owl:NamedIndividual rdf:about="http://purl.obolibrary.org/obo/GAZ_00076293">
        <obo:IAO_0000115>A national park in Botswana. Established 1971.</obo:IAO_0000115>
        <oboInOwl:hasOBONamespace>GAZ</oboInOwl:hasOBONamespace>
        <oboInOwl:id>GAZ:00076293</oboInOwl:id>
        <rdfs:label>Khutse Game Reserve</rdfs:label>
    </owl:NamedIndividual>
    


    <!-- http://purl.obolibrary.org/obo/GAZ_00076294 -->

    <owl:NamedIndividual rdf:about="http://purl.obolibrary.org/obo/GAZ_00076294">
        <obo:IAO_0000115>An area of Chobe National Park located at the Northwest corner of the park and to the North of Savuti, is adjacent to Linyanti River. To the west of this area lies Selinda Reserve and on the Northern bank of Kwando River is Namibia&apos;s Mamili National Park.</obo:IAO_0000115>
        <oboInOwl:hasOBONamespace>GAZ</oboInOwl:hasOBONamespace>
        <oboInOwl:id>GAZ:00076294</oboInOwl:id>
        <rdfs:label>Linyanti Marsh</rdfs:label>
    </owl:NamedIndividual>
    


    <!-- http://purl.obolibrary.org/obo/GAZ_00076641 -->

    <owl:NamedIndividual rdf:about="http://purl.obolibrary.org/obo/GAZ_00076641">
        <obo:IAO_0000115>One of the largest canyons in the world (definitely the largest in Africa). It features a gigantic ravine, in total about 160 km long, up to 27 km wide and in places almost 550 m deep.</obo:IAO_0000115>
        <oboInOwl:hasOBONamespace>GAZ</oboInOwl:hasOBONamespace>
        <oboInOwl:id>GAZ:00076641</oboInOwl:id>
        <rdfs:label>Fish River Canyon</rdfs:label>
    </owl:NamedIndividual>
    


    <!-- http://purl.obolibrary.org/obo/GAZ_00076643 -->

    <owl:NamedIndividual rdf:about="http://purl.obolibrary.org/obo/GAZ_00076643">
        <obo:IAO_0000115>An isolated Nature Reserve situated in the Kalahari Desert at the &apos;root&apos; of the Caprivi Strip in northeast of Namibia.</obo:IAO_0000115>
        <oboInOwl:hasOBONamespace>GAZ</oboInOwl:hasOBONamespace>
        <oboInOwl:id>GAZ:00076643</oboInOwl:id>
        <rdfs:label>Khaudom National Park</rdfs:label>
    </owl:NamedIndividual>
    


    <!-- http://purl.obolibrary.org/obo/GAZ_00076645 -->

    <owl:NamedIndividual rdf:about="http://purl.obolibrary.org/obo/GAZ_00076645">
        <obo:IAO_0000115>A national park in Namibia. Mamili is centered on the Nkasa and Lupala islands on the Kwando and Linyanti rivers in the south-western corner of East Caprivi.</obo:IAO_0000115>
        <oboInOwl:hasOBONamespace>GAZ</oboInOwl:hasOBONamespace>
        <oboInOwl:id>GAZ:00076645</oboInOwl:id>
        <rdfs:label>Mamili National Park</rdfs:label>
    </owl:NamedIndividual>
    


    <!-- http://purl.obolibrary.org/obo/GAZ_00076646 -->

    <owl:NamedIndividual rdf:about="http://purl.obolibrary.org/obo/GAZ_00076646">
        <obo:IAO_0000115>A national park in Namibia, created out of 1010 km2 of savannah, mopane woodlands, and marsh on the eastern shore of the Cuando River. Established 1990.</obo:IAO_0000115>
        <oboInOwl:hasOBONamespace>GAZ</oboInOwl:hasOBONamespace>
        <oboInOwl:id>GAZ:00076646</oboInOwl:id>
        <rdfs:label>Mudumu National Park</rdfs:label>
    </owl:NamedIndividual>
    


    <!-- http://purl.obolibrary.org/obo/GAZ_00076647 -->

    <owl:NamedIndividual rdf:about="http://purl.obolibrary.org/obo/GAZ_00076647">
        <obo:IAO_0000115>An ecological preserve in the Namib Desert.</obo:IAO_0000115>
        <oboInOwl:hasOBONamespace>GAZ</oboInOwl:hasOBONamespace>
        <oboInOwl:id>GAZ:00076647</oboInOwl:id>
        <rdfs:label>Namib-Naukluft National Park</rdfs:label>
    </owl:NamedIndividual>
    


    <!-- http://purl.obolibrary.org/obo/GAZ_00076649 -->

    <owl:NamedIndividual rdf:about="http://purl.obolibrary.org/obo/GAZ_00076649">
        <obo:RO_0001025 rdf:resource="http://purl.obolibrary.org/obo/GAZ_00014907"/>
        <oboInOwl:hasOBONamespace>GAZ</oboInOwl:hasOBONamespace>
        <oboInOwl:id>GAZ:00076649</oboInOwl:id>
        <rdfs:label>Waterberg Plateau</rdfs:label>
    </owl:NamedIndividual>
    


    <!-- http://purl.obolibrary.org/obo/GAZ_00076650 -->

    <owl:NamedIndividual rdf:about="http://purl.obolibrary.org/obo/GAZ_00076650">
        <obo:RO_0001025 rdf:resource="http://purl.obolibrary.org/obo/GAZ_00076649"/>
        <obo:IAO_0000115>A national park in central Namibia on the Waterberg Plateau, 68 km east of Otjiwarongo.</obo:IAO_0000115>
        <oboInOwl:hasOBONamespace>GAZ</oboInOwl:hasOBONamespace>
        <oboInOwl:id>GAZ:00076650</oboInOwl:id>
        <rdfs:label>Waterberg National Park</rdfs:label>
    </owl:NamedIndividual>
    


    <!-- http://purl.obolibrary.org/obo/GAZ_00135241 -->

    <owl:NamedIndividual rdf:about="http://purl.obolibrary.org/obo/GAZ_00135241">
        <obo:IAO_0000115>A dam on the Mazoe River in Zimbabwe, north of Harare. It was built mainly to provide irrigation for the Mazoe citrus estates. Constructed 1920.</obo:IAO_0000115>
        <oboInOwl:hasOBONamespace>GAZ</oboInOwl:hasOBONamespace>
        <oboInOwl:id>GAZ:00135241</oboInOwl:id>
        <rdfs:label>Mazoe Dam</rdfs:label>
    </owl:NamedIndividual>
    


    <!-- http://purl.obolibrary.org/obo/GAZ_00146586 -->

    <owl:NamedIndividual rdf:about="http://purl.obolibrary.org/obo/GAZ_00146586">
        <obo:RO_0001025 rdf:resource="http://purl.obolibrary.org/obo/GAZ_00032658"/>
        <obo:IAO_0000115>A small bay.</obo:IAO_0000115>
        <oboInOwl:hasOBONamespace>GAZ</oboInOwl:hasOBONamespace>
        <oboInOwl:id>GAZ:00146586</oboInOwl:id>
        <rdfs:label>Angra Pequena</rdfs:label>
    </owl:NamedIndividual>
    


    <!-- http://purl.obolibrary.org/obo/GAZ_00236226 -->

    <owl:NamedIndividual rdf:about="http://purl.obolibrary.org/obo/GAZ_00236226">
        <obo:IAO_0000115>An embankment dam with a hydroelectric power station and man-made lake near Kabwe, Zambia. Constructed 1950s.</obo:IAO_0000115>
        <oboInOwl:hasOBONamespace>GAZ</oboInOwl:hasOBONamespace>
        <oboInOwl:id>GAZ:00236226</oboInOwl:id>
        <rdfs:label>Mita Hills Dam</rdfs:label>
    </owl:NamedIndividual>
    


    <!-- http://purl.obolibrary.org/obo/GAZ_00237419 -->

    <owl:NamedIndividual rdf:about="http://purl.obolibrary.org/obo/GAZ_00237419">
        <obo:IAO_0000115>A river.</obo:IAO_0000115>
        <oboInOwl:hasOBONamespace>GAZ</oboInOwl:hasOBONamespace>
        <oboInOwl:id>GAZ:00237419</oboInOwl:id>
        <rdfs:label>Western Lunga River</rdfs:label>
    </owl:NamedIndividual>
    


    <!-- http://purl.obolibrary.org/obo/GAZ_00237426 -->

    <owl:NamedIndividual rdf:about="http://purl.obolibrary.org/obo/GAZ_00237426">
        <obo:RO_0001025 rdf:resource="http://purl.obolibrary.org/obo/GAZ_00076291"/>
        <obo:IAO_0000115>A large salt pan topographic depression which is part of the larger Makgadikgadi Pans in northeastern Botswana. This landform is a major part of the Nxai Pan National Park.</obo:IAO_0000115>
        <oboInOwl:hasOBONamespace>GAZ</oboInOwl:hasOBONamespace>
        <oboInOwl:id>GAZ:00237426</oboInOwl:id>
        <rdfs:label>Nxai Pan</rdfs:label>
    </owl:NamedIndividual>
    


    <!-- http://purl.obolibrary.org/obo/GAZ_00237427 -->

    <owl:NamedIndividual rdf:about="http://purl.obolibrary.org/obo/GAZ_00237427">
        <obo:RO_0001025 rdf:resource="http://purl.obolibrary.org/obo/GAZ_00075422"/>
        <obo:IAO_0000115>A large salt pan within the Makgadikgadi region of Botswana.</obo:IAO_0000115>
        <oboInOwl:hasOBONamespace>GAZ</oboInOwl:hasOBONamespace>
        <oboInOwl:id>GAZ:00237427</oboInOwl:id>
        <rdfs:label>Nwetwe Pan</rdfs:label>
    </owl:NamedIndividual>
    


    <!-- http://purl.obolibrary.org/obo/GAZ_00237428 -->

    <owl:NamedIndividual rdf:about="http://purl.obolibrary.org/obo/GAZ_00237428">
        <obo:RO_0001025 rdf:resource="http://purl.obolibrary.org/obo/GAZ_00075422"/>
        <obo:IAO_0000115>A large natural topographic depression within the Makgadikgadi region of Botswana. A seasonal lake.</obo:IAO_0000115>
        <oboInOwl:hasOBONamespace>GAZ</oboInOwl:hasOBONamespace>
        <oboInOwl:id>GAZ:00237428</oboInOwl:id>
        <rdfs:label>Sua Pan</rdfs:label>
    </owl:NamedIndividual>
    


    <!-- http://purl.obolibrary.org/obo/GAZ_00237429 -->

    <owl:NamedIndividual rdf:about="http://purl.obolibrary.org/obo/GAZ_00237429">
        <obo:RO_0001025 rdf:resource="http://purl.obolibrary.org/obo/GAZ_00016178"/>
        <obo:IAO_0000115>An island in Lake Kariba.</obo:IAO_0000115>
        <oboInOwl:hasOBONamespace>GAZ</oboInOwl:hasOBONamespace>
        <oboInOwl:id>GAZ:00237429</oboInOwl:id>
        <rdfs:label>Maaze Island</rdfs:label>
    </owl:NamedIndividual>
    


    <!-- http://purl.obolibrary.org/obo/GAZ_00237430 -->

    <owl:NamedIndividual rdf:about="http://purl.obolibrary.org/obo/GAZ_00237430">
        <obo:RO_0001025 rdf:resource="http://purl.obolibrary.org/obo/GAZ_00016178"/>
        <obo:IAO_0000115>An island in Lake Kariba.</obo:IAO_0000115>
        <oboInOwl:hasOBONamespace>GAZ</oboInOwl:hasOBONamespace>
        <oboInOwl:id>GAZ:00237430</oboInOwl:id>
        <rdfs:label>Mashape Island</rdfs:label>
    </owl:NamedIndividual>
    


    <!-- http://purl.obolibrary.org/obo/GAZ_00237431 -->

    <owl:NamedIndividual rdf:about="http://purl.obolibrary.org/obo/GAZ_00237431">
        <obo:RO_0001025 rdf:resource="http://purl.obolibrary.org/obo/GAZ_00016178"/>
        <obo:IAO_0000115>An island in Lake Kariba.</obo:IAO_0000115>
        <oboInOwl:hasOBONamespace>GAZ</oboInOwl:hasOBONamespace>
        <oboInOwl:id>GAZ:00237431</oboInOwl:id>
        <rdfs:label>Sampa Karuma Island</rdfs:label>
    </owl:NamedIndividual>
    


    <!-- http://purl.obolibrary.org/obo/GAZ_00237432 -->

    <owl:NamedIndividual rdf:about="http://purl.obolibrary.org/obo/GAZ_00237432">
        <obo:RO_0001025 rdf:resource="http://purl.obolibrary.org/obo/GAZ_00016178"/>
        <obo:IAO_0000115>An island in Lake Kariba.</obo:IAO_0000115>
        <oboInOwl:hasOBONamespace>GAZ</oboInOwl:hasOBONamespace>
        <oboInOwl:id>GAZ:00237432</oboInOwl:id>
        <rdfs:label>Fothergill Island</rdfs:label>
    </owl:NamedIndividual>
    


    <!-- http://purl.obolibrary.org/obo/GAZ_00237433 -->

    <owl:NamedIndividual rdf:about="http://purl.obolibrary.org/obo/GAZ_00237433">
        <obo:RO_0001025 rdf:resource="http://purl.obolibrary.org/obo/GAZ_00016178"/>
        <obo:IAO_0000115>An island in Lake Kariba.</obo:IAO_0000115>
        <oboInOwl:hasOBONamespace>GAZ</oboInOwl:hasOBONamespace>
        <oboInOwl:id>GAZ:00237433</oboInOwl:id>
        <rdfs:label>Spurwing Island</rdfs:label>
    </owl:NamedIndividual>
    


    <!-- http://purl.obolibrary.org/obo/GAZ_00237434 -->

    <owl:NamedIndividual rdf:about="http://purl.obolibrary.org/obo/GAZ_00237434">
        <obo:RO_0001025 rdf:resource="http://purl.obolibrary.org/obo/GAZ_00016178"/>
        <obo:IAO_0000115>An island in Lake Kariba.</obo:IAO_0000115>
        <oboInOwl:hasOBONamespace>GAZ</oboInOwl:hasOBONamespace>
        <oboInOwl:id>GAZ:00237434</oboInOwl:id>
        <rdfs:label>Snake Island</rdfs:label>
    </owl:NamedIndividual>
    


    <!-- http://purl.obolibrary.org/obo/GAZ_00237435 -->

    <owl:NamedIndividual rdf:about="http://purl.obolibrary.org/obo/GAZ_00237435">
        <obo:RO_0001025 rdf:resource="http://purl.obolibrary.org/obo/GAZ_00016178"/>
        <obo:IAO_0000115>An island in Lake Kariba.</obo:IAO_0000115>
        <oboInOwl:hasOBONamespace>GAZ</oboInOwl:hasOBONamespace>
        <oboInOwl:id>GAZ:00237435</oboInOwl:id>
        <rdfs:label>Antelope Island</rdfs:label>
    </owl:NamedIndividual>
    


    <!-- http://purl.obolibrary.org/obo/GAZ_00237436 -->

    <owl:NamedIndividual rdf:about="http://purl.obolibrary.org/obo/GAZ_00237436">
        <obo:RO_0001025 rdf:resource="http://purl.obolibrary.org/obo/GAZ_00016178"/>
        <obo:IAO_0000115>An island in Lake Kariba.</obo:IAO_0000115>
        <oboInOwl:hasOBONamespace>GAZ</oboInOwl:hasOBONamespace>
        <oboInOwl:id>GAZ:00237436</oboInOwl:id>
        <rdfs:label>Bed Island</rdfs:label>
    </owl:NamedIndividual>
    


    <!-- http://purl.obolibrary.org/obo/GAZ_00237437 -->

    <owl:NamedIndividual rdf:about="http://purl.obolibrary.org/obo/GAZ_00237437">
        <obo:RO_0001025 rdf:resource="http://purl.obolibrary.org/obo/GAZ_00016178"/>
        <obo:IAO_0000115>An island in Lake Kariba.</obo:IAO_0000115>
        <oboInOwl:hasOBONamespace>GAZ</oboInOwl:hasOBONamespace>
        <oboInOwl:id>GAZ:00237437</oboInOwl:id>
        <rdfs:label>Chikanka Island</rdfs:label>
    </owl:NamedIndividual>
    


    <!-- http://purl.obolibrary.org/obo/GAZ_00237440 -->

    <owl:NamedIndividual rdf:about="http://purl.obolibrary.org/obo/GAZ_00237440">
        <obo:IAO_0000115>A river. A tributary of the Kafue River.</obo:IAO_0000115>
        <oboInOwl:hasOBONamespace>GAZ</oboInOwl:hasOBONamespace>
        <oboInOwl:id>GAZ:00237440</oboInOwl:id>
        <rdfs:label>Lunga River</rdfs:label>
    </owl:NamedIndividual>
    


    <!-- http://purl.obolibrary.org/obo/GAZ_00237443 -->

    <owl:NamedIndividual rdf:about="http://purl.obolibrary.org/obo/GAZ_00237443">
        <obo:IAO_0000115>A dam. Constructed 1972.</obo:IAO_0000115>
        <oboInOwl:hasOBONamespace>GAZ</oboInOwl:hasOBONamespace>
        <oboInOwl:id>GAZ:00237443</oboInOwl:id>
        <rdfs:label>Kafue Gorge Dam</rdfs:label>
    </owl:NamedIndividual>
    


    <!-- http://purl.obolibrary.org/obo/GAZ_00237460 -->

    <owl:NamedIndividual rdf:about="http://purl.obolibrary.org/obo/GAZ_00237460">
        <obo:RO_0001025 rdf:resource="http://purl.obolibrary.org/obo/GAZ_00058785"/>
        <obo:IAO_0000115>A dam. Impounds Mulungushi Reservoir. Completed 1925.</obo:IAO_0000115>
        <oboInOwl:hasOBONamespace>GAZ</oboInOwl:hasOBONamespace>
        <oboInOwl:id>GAZ:00237460</oboInOwl:id>
        <rdfs:label>Mulungushi Dam</rdfs:label>
    </owl:NamedIndividual>
    


    <!-- http://purl.obolibrary.org/obo/GAZ_00237650 -->

    <owl:NamedIndividual rdf:about="http://purl.obolibrary.org/obo/GAZ_00237650">
        <obo:IAO_0000115>A dam.</obo:IAO_0000115>
        <oboInOwl:hasOBONamespace>GAZ</oboInOwl:hasOBONamespace>
        <oboInOwl:id>GAZ:00237650</oboInOwl:id>
        <rdfs:label>Ngezi Dam</rdfs:label>
    </owl:NamedIndividual>
    


    <!-- http://purl.obolibrary.org/obo/GAZ_00237862 -->

    <owl:NamedIndividual rdf:about="http://purl.obolibrary.org/obo/GAZ_00237862">
        <obo:IAO_0000115>A river.</obo:IAO_0000115>
        <oboInOwl:hasOBONamespace>GAZ</oboInOwl:hasOBONamespace>
        <oboInOwl:id>GAZ:00237862</oboInOwl:id>
        <rdfs:label>Utembo River</rdfs:label>
    </owl:NamedIndividual>
    


    <!-- http://purl.obolibrary.org/obo/GAZ_00237960 -->

    <owl:NamedIndividual rdf:about="http://purl.obolibrary.org/obo/GAZ_00237960">
        <obo:RO_0001025 rdf:resource="http://purl.obolibrary.org/obo/GAZ_00032700"/>
        <obo:IAO_0000115>A dam on the Kunene River outside of Oshakati, Oshana Region, Namibia.</obo:IAO_0000115>
        <oboInOwl:hasOBONamespace>GAZ</oboInOwl:hasOBONamespace>
        <oboInOwl:id>GAZ:00237960</oboInOwl:id>
        <rdfs:label>Olushandja Dam</rdfs:label>
    </owl:NamedIndividual>
    


    <!-- http://purl.obolibrary.org/obo/GAZ_00237961 -->

    <owl:NamedIndividual rdf:about="http://purl.obolibrary.org/obo/GAZ_00237961">
        <obo:IAO_0000115>A dam.</obo:IAO_0000115>
        <oboInOwl:hasOBONamespace>GAZ</oboInOwl:hasOBONamespace>
        <oboInOwl:id>GAZ:00237961</oboInOwl:id>
        <rdfs:label>Barragem do Ruacana</rdfs:label>
    </owl:NamedIndividual>
    


    <!-- http://purl.obolibrary.org/obo/GAZ_00238410 -->

    <owl:NamedIndividual rdf:about="http://purl.obolibrary.org/obo/GAZ_00238410">
        <obo:IAO_0000115>A desert.</obo:IAO_0000115>
        <oboInOwl:hasOBONamespace>GAZ</oboInOwl:hasOBONamespace>
        <oboInOwl:id>GAZ:00238410</oboInOwl:id>
        <rdfs:label>Mossamedes Desert</rdfs:label>
    </owl:NamedIndividual>
    


    <!-- http://purl.obolibrary.org/obo/GAZ_00238416 -->

    <owl:NamedIndividual rdf:about="http://purl.obolibrary.org/obo/GAZ_00238416">
        <obo:IAO_0000115>A lake located to the south of the Boteti River and the Makgadikgadi Pans, was once a large shallow lake fed by overspill from the Boteti River. However, since the impoundment at Mopipi, itself a former pan, the lake is usually as dry as the pans in nearby Makgadikgadi Depression.</obo:IAO_0000115>
        <oboInOwl:hasOBONamespace>GAZ</oboInOwl:hasOBONamespace>
        <oboInOwl:id>GAZ:00238416</oboInOwl:id>
        <rdfs:label>Lake Xau</rdfs:label>
    </owl:NamedIndividual>
    


    <!-- http://purl.obolibrary.org/obo/GAZ_00238777 -->

    <owl:NamedIndividual rdf:about="http://purl.obolibrary.org/obo/GAZ_00238777">
        <obo:RO_0001025 rdf:resource="http://purl.obolibrary.org/obo/GAZ_00014899"/>
        <obo:IAO_0000115>A headwater of the Nossob River.</obo:IAO_0000115>
        <oboInOwl:hasOBONamespace>GAZ</oboInOwl:hasOBONamespace>
        <oboInOwl:id>GAZ:00238777</oboInOwl:id>
        <rdfs:label>Swart-Nossob River</rdfs:label>
    </owl:NamedIndividual>
    


    <!-- http://purl.obolibrary.org/obo/GAZ_00238778 -->

    <owl:NamedIndividual rdf:about="http://purl.obolibrary.org/obo/GAZ_00238778">
        <obo:RO_0001025 rdf:resource="http://purl.obolibrary.org/obo/GAZ_00014899"/>
        <obo:IAO_0000115>A headwater of the Nossob River.</obo:IAO_0000115>
        <oboInOwl:hasOBONamespace>GAZ</oboInOwl:hasOBONamespace>
        <oboInOwl:id>GAZ:00238778</oboInOwl:id>
        <rdfs:label>Wit-Nossob River</rdfs:label>
    </owl:NamedIndividual>
    


    <!-- http://purl.obolibrary.org/obo/GAZ_00238779 -->

    <owl:NamedIndividual rdf:about="http://purl.obolibrary.org/obo/GAZ_00238779">
        <obo:RO_0001025 rdf:resource="http://purl.obolibrary.org/obo/GAZ_00014908"/>
        <obo:IAO_0000115>A river. A tributary of the Nossob River.</obo:IAO_0000115>
        <oboInOwl:hasOBONamespace>GAZ</oboInOwl:hasOBONamespace>
        <oboInOwl:id>GAZ:00238779</oboInOwl:id>
        <rdfs:label>Auob River</rdfs:label>
    </owl:NamedIndividual>
    


    <!-- http://purl.obolibrary.org/obo/GAZ_00238782 -->

    <owl:NamedIndividual rdf:about="http://purl.obolibrary.org/obo/GAZ_00238782">
        <obo:RO_0001025 rdf:resource="http://purl.obolibrary.org/obo/GAZ_00237428"/>
        <obo:IAO_0000115>An igneous rock island in Sua Pan.</obo:IAO_0000115>
        <oboInOwl:hasOBONamespace>GAZ</oboInOwl:hasOBONamespace>
        <oboInOwl:id>GAZ:00238782</oboInOwl:id>
        <rdfs:label>Kukome Island</rdfs:label>
    </owl:NamedIndividual>
    


    <!-- http://purl.obolibrary.org/obo/GAZ_00238896 -->

    <owl:NamedIndividual rdf:about="http://purl.obolibrary.org/obo/GAZ_00238896">
        <obo:IAO_0000115>An island in the Chobe River on the border between Namibia and Botswana, near the Botswanan town of Kasane. It was the subject of a territorial dispute between these countries, resolved by a 1999 decision of the International Court of Justice which ruled in favour of Botswana.</obo:IAO_0000115>
        <oboInOwl:hasOBONamespace>GAZ</oboInOwl:hasOBONamespace>
        <oboInOwl:id>GAZ:00238896</oboInOwl:id>
        <rdfs:label>Kasikili Island</rdfs:label>
    </owl:NamedIndividual>
    


    <!-- http://purl.obolibrary.org/obo/GAZ_00238901 -->

    <owl:NamedIndividual rdf:about="http://purl.obolibrary.org/obo/GAZ_00238901">
        <obo:IAO_0000115>Pans located SW of the Makgadikgadi Pans.</obo:IAO_0000115>
        <oboInOwl:hasOBONamespace>GAZ</oboInOwl:hasOBONamespace>
        <oboInOwl:id>GAZ:00238901</oboInOwl:id>
        <rdfs:label>Deception Pans</rdfs:label>
    </owl:NamedIndividual>
    


    <!-- http://purl.obolibrary.org/obo/GAZ_00238904 -->

    <owl:NamedIndividual rdf:about="http://purl.obolibrary.org/obo/GAZ_00238904">
        <obo:IAO_0000115>A dam.</obo:IAO_0000115>
        <oboInOwl:hasOBONamespace>GAZ</oboInOwl:hasOBONamespace>
        <oboInOwl:id>GAZ:00238904</oboInOwl:id>
        <rdfs:label>Muela Dam</rdfs:label>
    </owl:NamedIndividual>
    


    <!-- http://purl.obolibrary.org/obo/GAZ_00238915 -->

    <owl:NamedIndividual rdf:about="http://purl.obolibrary.org/obo/GAZ_00238915">
        <obo:IAO_0000115>A river in northern Lesotho. It flows south from close to the South African border, past the town of Ha Lejone and joins the Senqu River close to the town of Taung.</obo:IAO_0000115>
        <oboInOwl:hasOBONamespace>GAZ</oboInOwl:hasOBONamespace>
        <oboInOwl:id>GAZ:00238915</oboInOwl:id>
        <rdfs:label>Malibamat&apos;so River</rdfs:label>
    </owl:NamedIndividual>
    


    <!-- http://purl.obolibrary.org/obo/GAZ_00239433 -->

    <owl:NamedIndividual rdf:about="http://purl.obolibrary.org/obo/GAZ_00239433">
        <obo:RO_0001025 rdf:resource="http://purl.obolibrary.org/obo/GAZ_00076645"/>
        <obo:IAO_0000115>An island.</obo:IAO_0000115>
        <oboInOwl:hasOBONamespace>GAZ</oboInOwl:hasOBONamespace>
        <oboInOwl:id>GAZ:00239433</oboInOwl:id>
        <rdfs:label>Nkasa Island</rdfs:label>
    </owl:NamedIndividual>
    


    <!-- http://purl.obolibrary.org/obo/GAZ_00239434 -->

    <owl:NamedIndividual rdf:about="http://purl.obolibrary.org/obo/GAZ_00239434">
        <obo:RO_0001025 rdf:resource="http://purl.obolibrary.org/obo/GAZ_00076645"/>
        <obo:IAO_0000115>An island.</obo:IAO_0000115>
        <oboInOwl:hasOBONamespace>GAZ</oboInOwl:hasOBONamespace>
        <oboInOwl:id>GAZ:00239434</oboInOwl:id>
        <rdfs:label>Lupala island</rdfs:label>
    </owl:NamedIndividual>
    


    <!-- http://purl.obolibrary.org/obo/GAZ_00239435 -->

    <owl:NamedIndividual rdf:about="http://purl.obolibrary.org/obo/GAZ_00239435">
        <obo:IAO_0000115>A protected area.</obo:IAO_0000115>
        <oboInOwl:hasOBONamespace>GAZ</oboInOwl:hasOBONamespace>
        <oboInOwl:id>GAZ:00239435</oboInOwl:id>
        <rdfs:label>Bwabwata National Park</rdfs:label>
    </owl:NamedIndividual>
    


    <!-- http://purl.obolibrary.org/obo/GAZ_00239436 -->

    <owl:NamedIndividual rdf:about="http://purl.obolibrary.org/obo/GAZ_00239436">
        <obo:IAO_0000115>A protected area.</obo:IAO_0000115>
        <oboInOwl:hasOBONamespace>GAZ</oboInOwl:hasOBONamespace>
        <oboInOwl:id>GAZ:00239436</oboInOwl:id>
        <rdfs:label>Mahango Game Reserve</rdfs:label>
    </owl:NamedIndividual>
    


    <!-- http://purl.obolibrary.org/obo/GAZ_00239437 -->

    <owl:NamedIndividual rdf:about="http://purl.obolibrary.org/obo/GAZ_00239437">
        <obo:IAO_0000115>A freshwater lake. A wide part of the Cuando River.</obo:IAO_0000115>
        <oboInOwl:hasOBONamespace>GAZ</oboInOwl:hasOBONamespace>
        <oboInOwl:id>GAZ:00239437</oboInOwl:id>
        <rdfs:label>Liambezi Lake</rdfs:label>
    </owl:NamedIndividual>
    


    <!-- http://purl.obolibrary.org/obo/GAZ_00239439 -->

    <owl:NamedIndividual rdf:about="http://purl.obolibrary.org/obo/GAZ_00239439">
        <obo:IAO_0000115>An emphemeral river in the western part of Namibia. Discharges to the Atlantic Ocean.</obo:IAO_0000115>
        <oboInOwl:hasOBONamespace>GAZ</oboInOwl:hasOBONamespace>
        <oboInOwl:id>GAZ:00239439</oboInOwl:id>
        <rdfs:label>Swakop River</rdfs:label>
    </owl:NamedIndividual>
    


    <!-- http://purl.obolibrary.org/obo/GAZ_00239440 -->

    <owl:NamedIndividual rdf:about="http://purl.obolibrary.org/obo/GAZ_00239440">
        <rdf:type rdf:resource="http://purl.obolibrary.org/obo/ENVO_00000167"/>
        <obo:RO_0001025 rdf:resource="http://purl.obolibrary.org/obo/GAZ_00032643"/>
        <obo:IAO_0000115>A sand spit.</obo:IAO_0000115>
        <oboInOwl:hasOBONamespace>GAZ</oboInOwl:hasOBONamespace>
        <oboInOwl:id>GAZ:00239440</oboInOwl:id>
        <rdfs:label>Pelican Point</rdfs:label>
    </owl:NamedIndividual>
    


    <!-- http://purl.obolibrary.org/obo/GAZ_00239442 -->

    <owl:NamedIndividual rdf:about="http://purl.obolibrary.org/obo/GAZ_00239442">
        <obo:RO_0001025 rdf:resource="http://purl.obolibrary.org/obo/GAZ_00239526"/>
        <obo:IAO_0000115>A dam close to Mariental, Hardap Region, Namibia.</obo:IAO_0000115>
        <oboInOwl:hasOBONamespace>GAZ</oboInOwl:hasOBONamespace>
        <oboInOwl:id>GAZ:00239442</oboInOwl:id>
        <rdfs:label>Hardap Dam</rdfs:label>
    </owl:NamedIndividual>
    


    <!-- http://purl.obolibrary.org/obo/GAZ_00239443 -->

    <owl:NamedIndividual rdf:about="http://purl.obolibrary.org/obo/GAZ_00239443">
        <obo:RO_0001025 rdf:resource="http://purl.obolibrary.org/obo/GAZ_00014900"/>
        <obo:IAO_0000115>A mountain range in the S of the Karas Region.</obo:IAO_0000115>
        <oboInOwl:hasOBONamespace>GAZ</oboInOwl:hasOBONamespace>
        <oboInOwl:id>GAZ:00239443</oboInOwl:id>
        <rdfs:label>Karas Mountain Range</rdfs:label>
    </owl:NamedIndividual>
    


    <!-- http://purl.obolibrary.org/obo/GAZ_00239444 -->

    <owl:NamedIndividual rdf:about="http://purl.obolibrary.org/obo/GAZ_00239444">
        <obo:RO_0001025 rdf:resource="http://purl.obolibrary.org/obo/GAZ_00239455"/>
        <obo:IAO_0000115>A constituency in Katutura, Windhoek, Khomas Region, Namibia.</obo:IAO_0000115>
        <oboInOwl:hasOBONamespace>GAZ</oboInOwl:hasOBONamespace>
        <oboInOwl:id>GAZ:00239444</oboInOwl:id>
        <rdfs:label>Moses Garoeb Constituency</rdfs:label>
    </owl:NamedIndividual>
    


    <!-- http://purl.obolibrary.org/obo/GAZ_00239445 -->

    <owl:NamedIndividual rdf:about="http://purl.obolibrary.org/obo/GAZ_00239445">
        <obo:RO_0001025 rdf:resource="http://purl.obolibrary.org/obo/GAZ_00239455"/>
        <obo:IAO_0000115>A constituency in Katutura, Windhoek, Khomas Region, Namibia.</obo:IAO_0000115>
        <oboInOwl:hasOBONamespace>GAZ</oboInOwl:hasOBONamespace>
        <oboInOwl:id>GAZ:00239445</oboInOwl:id>
        <rdfs:label>Tobias Hainyeko Constituency</rdfs:label>
    </owl:NamedIndividual>
    


    <!-- http://purl.obolibrary.org/obo/GAZ_00239446 -->

    <owl:NamedIndividual rdf:about="http://purl.obolibrary.org/obo/GAZ_00239446">
        <obo:RO_0001025 rdf:resource="http://purl.obolibrary.org/obo/GAZ_00014898"/>
        <obo:IAO_0000115>The capital city of Namibia.</obo:IAO_0000115>
        <oboInOwl:hasOBONamespace>GAZ</oboInOwl:hasOBONamespace>
        <oboInOwl:id>GAZ:00239446</oboInOwl:id>
        <rdfs:label>Windhoek</rdfs:label>
    </owl:NamedIndividual>
    


    <!-- http://purl.obolibrary.org/obo/GAZ_00239447 -->

    <owl:NamedIndividual rdf:about="http://purl.obolibrary.org/obo/GAZ_00239447">
        <obo:RO_0001025 rdf:resource="http://purl.obolibrary.org/obo/GAZ_00032660"/>
        <obo:IAO_0000115>A suburb of Windhoek.</obo:IAO_0000115>
        <oboInOwl:hasOBONamespace>GAZ</oboInOwl:hasOBONamespace>
        <oboInOwl:id>GAZ:00239447</oboInOwl:id>
        <rdfs:label>Academia</rdfs:label>
    </owl:NamedIndividual>
    


    <!-- http://purl.obolibrary.org/obo/GAZ_00239448 -->

    <owl:NamedIndividual rdf:about="http://purl.obolibrary.org/obo/GAZ_00239448">
        <obo:RO_0001025 rdf:resource="http://purl.obolibrary.org/obo/GAZ_00239446"/>
        <obo:IAO_0000115>A suburb of Windhoek.</obo:IAO_0000115>
        <oboInOwl:hasOBONamespace>GAZ</oboInOwl:hasOBONamespace>
        <oboInOwl:id>GAZ:00239448</oboInOwl:id>
        <rdfs:label>Auasblick</rdfs:label>
    </owl:NamedIndividual>
    


    <!-- http://purl.obolibrary.org/obo/GAZ_00239449 -->

    <owl:NamedIndividual rdf:about="http://purl.obolibrary.org/obo/GAZ_00239449">
        <obo:RO_0001025 rdf:resource="http://purl.obolibrary.org/obo/GAZ_00239446"/>
        <obo:IAO_0000115>A suburb of Windhoek.</obo:IAO_0000115>
        <oboInOwl:hasOBONamespace>GAZ</oboInOwl:hasOBONamespace>
        <oboInOwl:id>GAZ:00239449</oboInOwl:id>
        <rdfs:label>Avis</rdfs:label>
    </owl:NamedIndividual>
    


    <!-- http://purl.obolibrary.org/obo/GAZ_00239450 -->

    <owl:NamedIndividual rdf:about="http://purl.obolibrary.org/obo/GAZ_00239450">
        <obo:RO_0001025 rdf:resource="http://purl.obolibrary.org/obo/GAZ_00032660"/>
        <obo:IAO_0000115>A suburb of Windhoek.</obo:IAO_0000115>
        <oboInOwl:hasOBONamespace>GAZ</oboInOwl:hasOBONamespace>
        <oboInOwl:id>GAZ:00239450</oboInOwl:id>
        <rdfs:label>Cimbebasia</rdfs:label>
    </owl:NamedIndividual>
    


    <!-- http://purl.obolibrary.org/obo/GAZ_00239451 -->

    <owl:NamedIndividual rdf:about="http://purl.obolibrary.org/obo/GAZ_00239451">
        <obo:RO_0001025 rdf:resource="http://purl.obolibrary.org/obo/GAZ_00239446"/>
        <obo:IAO_0000115>A suburb of Windhoek.</obo:IAO_0000115>
        <oboInOwl:hasOBONamespace>GAZ</oboInOwl:hasOBONamespace>
        <oboInOwl:id>GAZ:00239451</oboInOwl:id>
        <rdfs:label>Dorado Park</rdfs:label>
    </owl:NamedIndividual>
    


    <!-- http://purl.obolibrary.org/obo/GAZ_00239452 -->

    <owl:NamedIndividual rdf:about="http://purl.obolibrary.org/obo/GAZ_00239452">
        <obo:RO_0001025 rdf:resource="http://purl.obolibrary.org/obo/GAZ_00239446"/>
        <obo:IAO_0000115>A suburb of Windhoek.</obo:IAO_0000115>
        <oboInOwl:hasOBONamespace>GAZ</oboInOwl:hasOBONamespace>
        <oboInOwl:id>GAZ:00239452</oboInOwl:id>
        <rdfs:label>Eros</rdfs:label>
    </owl:NamedIndividual>
    


    <!-- http://purl.obolibrary.org/obo/GAZ_00239453 -->

    <owl:NamedIndividual rdf:about="http://purl.obolibrary.org/obo/GAZ_00239453">
        <obo:RO_0001025 rdf:resource="http://purl.obolibrary.org/obo/GAZ_00239446"/>
        <obo:IAO_0000115>A suburb of Windhoek.</obo:IAO_0000115>
        <oboInOwl:hasOBONamespace>GAZ</oboInOwl:hasOBONamespace>
        <oboInOwl:id>GAZ:00239453</oboInOwl:id>
        <rdfs:label>Eros Park</rdfs:label>
    </owl:NamedIndividual>
    


    <!-- http://purl.obolibrary.org/obo/GAZ_00239454 -->

    <owl:NamedIndividual rdf:about="http://purl.obolibrary.org/obo/GAZ_00239454">
        <obo:RO_0001025 rdf:resource="http://purl.obolibrary.org/obo/GAZ_00239446"/>
        <obo:IAO_0000115>A suburb of Windhoek.</obo:IAO_0000115>
        <oboInOwl:hasOBONamespace>GAZ</oboInOwl:hasOBONamespace>
        <oboInOwl:id>GAZ:00239454</oboInOwl:id>
        <rdfs:label>Goreangab</rdfs:label>
    </owl:NamedIndividual>
    


    <!-- http://purl.obolibrary.org/obo/GAZ_00239455 -->

    <owl:NamedIndividual rdf:about="http://purl.obolibrary.org/obo/GAZ_00239455">
        <obo:RO_0001025 rdf:resource="http://purl.obolibrary.org/obo/GAZ_00239446"/>
        <obo:IAO_0000115>A suburb of Windhoek, the capital of Namibia. The township is situated in the north of the town between the suburbs of Katutura, Wanaheda, and Okuryangava.</obo:IAO_0000115>
        <oboInOwl:hasOBONamespace>GAZ</oboInOwl:hasOBONamespace>
        <oboInOwl:id>GAZ:00239455</oboInOwl:id>
        <rdfs:label>Hakahana</rdfs:label>
    </owl:NamedIndividual>
    


    <!-- http://purl.obolibrary.org/obo/GAZ_00239456 -->

    <owl:NamedIndividual rdf:about="http://purl.obolibrary.org/obo/GAZ_00239456">
        <obo:RO_0001025 rdf:resource="http://purl.obolibrary.org/obo/GAZ_00032660"/>
        <obo:IAO_0000115>A residential suburb in Windhoek, the capital of Namibia.</obo:IAO_0000115>
        <oboInOwl:hasOBONamespace>GAZ</oboInOwl:hasOBONamespace>
        <oboInOwl:id>GAZ:00239456</oboInOwl:id>
        <rdfs:label>Hochland Park</rdfs:label>
    </owl:NamedIndividual>
    


    <!-- http://purl.obolibrary.org/obo/GAZ_00239457 -->

    <owl:NamedIndividual rdf:about="http://purl.obolibrary.org/obo/GAZ_00239457">
        <obo:RO_0001025 rdf:resource="http://purl.obolibrary.org/obo/GAZ_00239446"/>
        <obo:IAO_0000115>A populated place. A township of Windhoek, Khomas Region, Namibia.</obo:IAO_0000115>
        <oboInOwl:hasOBONamespace>GAZ</oboInOwl:hasOBONamespace>
        <oboInOwl:id>GAZ:00239457</oboInOwl:id>
        <rdfs:label>Katutura</rdfs:label>
    </owl:NamedIndividual>
    


    <!-- http://purl.obolibrary.org/obo/GAZ_00239458 -->

    <owl:NamedIndividual rdf:about="http://purl.obolibrary.org/obo/GAZ_00239458">
        <obo:RO_0001025 rdf:resource="http://purl.obolibrary.org/obo/GAZ_00239446"/>
        <obo:IAO_0000115>A suburb of Namibia&apos;s capital of Windhoek in the Khomas Region.</obo:IAO_0000115>
        <oboInOwl:hasOBONamespace>GAZ</oboInOwl:hasOBONamespace>
        <oboInOwl:id>GAZ:00239458</oboInOwl:id>
        <rdfs:label>Khomasdal</rdfs:label>
    </owl:NamedIndividual>
    


    <!-- http://purl.obolibrary.org/obo/GAZ_00239459 -->

    <owl:NamedIndividual rdf:about="http://purl.obolibrary.org/obo/GAZ_00239459">
        <obo:RO_0001025 rdf:resource="http://purl.obolibrary.org/obo/GAZ_00239446"/>
        <obo:IAO_0000115>A suburb of Windhoek.</obo:IAO_0000115>
        <oboInOwl:hasOBONamespace>GAZ</oboInOwl:hasOBONamespace>
        <oboInOwl:id>GAZ:00239459</oboInOwl:id>
        <rdfs:label>Kleine Kuppe</rdfs:label>
    </owl:NamedIndividual>
    


    <!-- http://purl.obolibrary.org/obo/GAZ_00239460 -->

    <owl:NamedIndividual rdf:about="http://purl.obolibrary.org/obo/GAZ_00239460">
        <obo:RO_0001025 rdf:resource="http://purl.obolibrary.org/obo/GAZ_00239446"/>
        <obo:IAO_0000115>A suburb of Windhoek.</obo:IAO_0000115>
        <oboInOwl:hasOBONamespace>GAZ</oboInOwl:hasOBONamespace>
        <oboInOwl:id>GAZ:00239460</oboInOwl:id>
        <rdfs:label>Klein-Windhoek</rdfs:label>
    </owl:NamedIndividual>
    


    <!-- http://purl.obolibrary.org/obo/GAZ_00239461 -->

    <owl:NamedIndividual rdf:about="http://purl.obolibrary.org/obo/GAZ_00239461">
        <obo:RO_0001025 rdf:resource="http://purl.obolibrary.org/obo/GAZ_00239446"/>
        <obo:IAO_0000115>A suburb of Windhoek.</obo:IAO_0000115>
        <oboInOwl:hasOBONamespace>GAZ</oboInOwl:hasOBONamespace>
        <oboInOwl:id>GAZ:00239461</oboInOwl:id>
        <rdfs:label>Lafrenz Industrial Area</rdfs:label>
    </owl:NamedIndividual>
    


    <!-- http://purl.obolibrary.org/obo/GAZ_00239462 -->

    <owl:NamedIndividual rdf:about="http://purl.obolibrary.org/obo/GAZ_00239462">
        <obo:RO_0001025 rdf:resource="http://purl.obolibrary.org/obo/GAZ_00239446"/>
        <obo:IAO_0000115>A suburb of Windhoek.</obo:IAO_0000115>
        <oboInOwl:hasOBONamespace>GAZ</oboInOwl:hasOBONamespace>
        <oboInOwl:id>GAZ:00239462</oboInOwl:id>
        <rdfs:label>Ludwigsdorf</rdfs:label>
    </owl:NamedIndividual>
    


    <!-- http://purl.obolibrary.org/obo/GAZ_00239463 -->

    <owl:NamedIndividual rdf:about="http://purl.obolibrary.org/obo/GAZ_00239463">
        <obo:RO_0001025 rdf:resource="http://purl.obolibrary.org/obo/GAZ_00239446"/>
        <obo:IAO_0000115>A suburb of Windhoek.</obo:IAO_0000115>
        <oboInOwl:hasOBONamespace>GAZ</oboInOwl:hasOBONamespace>
        <oboInOwl:id>GAZ:00239463</oboInOwl:id>
        <rdfs:label>Luxury Hill</rdfs:label>
    </owl:NamedIndividual>
    


    <!-- http://purl.obolibrary.org/obo/GAZ_00239464 -->

    <owl:NamedIndividual rdf:about="http://purl.obolibrary.org/obo/GAZ_00239464">
        <obo:RO_0001025 rdf:resource="http://purl.obolibrary.org/obo/GAZ_00239446"/>
        <obo:IAO_0000115>A suburb of Windhoek.</obo:IAO_0000115>
        <oboInOwl:hasOBONamespace>GAZ</oboInOwl:hasOBONamespace>
        <oboInOwl:id>GAZ:00239464</oboInOwl:id>
        <rdfs:label>Northern Industrial</rdfs:label>
    </owl:NamedIndividual>
    


    <!-- http://purl.obolibrary.org/obo/GAZ_00239465 -->

    <owl:NamedIndividual rdf:about="http://purl.obolibrary.org/obo/GAZ_00239465">
        <obo:RO_0001025 rdf:resource="http://purl.obolibrary.org/obo/GAZ_00239446"/>
        <obo:IAO_0000115>A suburb of Windhoek.</obo:IAO_0000115>
        <oboInOwl:hasOBONamespace>GAZ</oboInOwl:hasOBONamespace>
        <oboInOwl:id>GAZ:00239465</oboInOwl:id>
        <rdfs:label>Olympia</rdfs:label>
    </owl:NamedIndividual>
    


    <!-- http://purl.obolibrary.org/obo/GAZ_00239466 -->

    <owl:NamedIndividual rdf:about="http://purl.obolibrary.org/obo/GAZ_00239466">
        <obo:RO_0001025 rdf:resource="http://purl.obolibrary.org/obo/GAZ_00239446"/>
        <obo:IAO_0000115>A populated place. A township in north-western Windhoek, Namibia.</obo:IAO_0000115>
        <oboInOwl:hasOBONamespace>GAZ</oboInOwl:hasOBONamespace>
        <oboInOwl:id>GAZ:00239466</oboInOwl:id>
        <rdfs:label>Otjomuise</rdfs:label>
    </owl:NamedIndividual>
    


    <!-- http://purl.obolibrary.org/obo/GAZ_00239467 -->

    <owl:NamedIndividual rdf:about="http://purl.obolibrary.org/obo/GAZ_00239467">
        <obo:RO_0001025 rdf:resource="http://purl.obolibrary.org/obo/GAZ_00032660"/>
        <obo:IAO_0000115>A suburb in the south of Windhoek, Namibia, in the Windhoek West parliamentary consituency.</obo:IAO_0000115>
        <oboInOwl:hasOBONamespace>GAZ</oboInOwl:hasOBONamespace>
        <oboInOwl:id>GAZ:00239467</oboInOwl:id>
        <rdfs:label>Pioneers Park</rdfs:label>
    </owl:NamedIndividual>
    


    <!-- http://purl.obolibrary.org/obo/GAZ_00239468 -->

    <owl:NamedIndividual rdf:about="http://purl.obolibrary.org/obo/GAZ_00239468">
        <obo:RO_0001025 rdf:resource="http://purl.obolibrary.org/obo/GAZ_00239446"/>
        <obo:IAO_0000115>A suburb of Windhoek.</obo:IAO_0000115>
        <oboInOwl:hasOBONamespace>GAZ</oboInOwl:hasOBONamespace>
        <oboInOwl:id>GAZ:00239468</oboInOwl:id>
        <rdfs:label>Prosperita</rdfs:label>
    </owl:NamedIndividual>
    


    <!-- http://purl.obolibrary.org/obo/GAZ_00239469 -->

    <owl:NamedIndividual rdf:about="http://purl.obolibrary.org/obo/GAZ_00239469">
        <obo:RO_0001025 rdf:resource="http://purl.obolibrary.org/obo/GAZ_00032660"/>
        <obo:IAO_0000115>A suburb of Windhoek.</obo:IAO_0000115>
        <oboInOwl:hasOBONamespace>GAZ</oboInOwl:hasOBONamespace>
        <oboInOwl:id>GAZ:00239469</oboInOwl:id>
        <rdfs:label>Rocky Crest</rdfs:label>
    </owl:NamedIndividual>
    


    <!-- http://purl.obolibrary.org/obo/GAZ_00239470 -->

    <owl:NamedIndividual rdf:about="http://purl.obolibrary.org/obo/GAZ_00239470">
        <obo:RO_0001025 rdf:resource="http://purl.obolibrary.org/obo/GAZ_00239446"/>
        <obo:IAO_0000115>A suburb of Windhoek.</obo:IAO_0000115>
        <oboInOwl:hasOBONamespace>GAZ</oboInOwl:hasOBONamespace>
        <oboInOwl:id>GAZ:00239470</oboInOwl:id>
        <rdfs:label>Southern Industrial</rdfs:label>
    </owl:NamedIndividual>
    


    <!-- http://purl.obolibrary.org/obo/GAZ_00239471 -->

    <owl:NamedIndividual rdf:about="http://purl.obolibrary.org/obo/GAZ_00239471">
        <obo:RO_0001025 rdf:resource="http://purl.obolibrary.org/obo/GAZ_00239446"/>
        <obo:IAO_0000115>A suburb of Windhoek.</obo:IAO_0000115>
        <oboInOwl:hasOBONamespace>GAZ</oboInOwl:hasOBONamespace>
        <oboInOwl:id>GAZ:00239471</oboInOwl:id>
        <rdfs:label>Suiderhof</rdfs:label>
    </owl:NamedIndividual>
    


    <!-- http://purl.obolibrary.org/obo/GAZ_00239472 -->

    <owl:NamedIndividual rdf:about="http://purl.obolibrary.org/obo/GAZ_00239472">
        <obo:RO_0001025 rdf:resource="http://purl.obolibrary.org/obo/GAZ_00239446"/>
        <obo:IAO_0000115>A suburb of Windhoek.</obo:IAO_0000115>
        <oboInOwl:hasOBONamespace>GAZ</oboInOwl:hasOBONamespace>
        <oboInOwl:id>GAZ:00239472</oboInOwl:id>
        <rdfs:label>Wanaheda</rdfs:label>
    </owl:NamedIndividual>
    


    <!-- http://purl.obolibrary.org/obo/GAZ_00239473 -->

    <owl:NamedIndividual rdf:about="http://purl.obolibrary.org/obo/GAZ_00239473">
        <obo:RO_0001025 rdf:resource="http://purl.obolibrary.org/obo/GAZ_00239446"/>
        <obo:IAO_0000115>The inner city area of Windhoek, capital of Namibia. It is surrounded by the suburbs of Windhoek West and Hochland Park in the west, Windhoek-North in the north, Eros, Klein-Windhoek, Luxushugel and Auasblick in the east, and Suiderhof and Southern Industrial in the south.</obo:IAO_0000115>
        <oboInOwl:hasOBONamespace>GAZ</oboInOwl:hasOBONamespace>
        <oboInOwl:id>GAZ:00239473</oboInOwl:id>
        <rdfs:label>Windhoek Central Business District</rdfs:label>
    </owl:NamedIndividual>
    


    <!-- http://purl.obolibrary.org/obo/GAZ_00239474 -->

    <owl:NamedIndividual rdf:about="http://purl.obolibrary.org/obo/GAZ_00239474">
        <obo:RO_0001025 rdf:resource="http://purl.obolibrary.org/obo/GAZ_00032660"/>
        <oboInOwl:hasOBONamespace>GAZ</oboInOwl:hasOBONamespace>
        <oboInOwl:id>GAZ:00239474</oboInOwl:id>
        <rdfs:label>Windhoek North</rdfs:label>
    </owl:NamedIndividual>
    


    <!-- http://purl.obolibrary.org/obo/GAZ_00239475 -->

    <owl:NamedIndividual rdf:about="http://purl.obolibrary.org/obo/GAZ_00239475">
        <obo:RO_0001025 rdf:resource="http://purl.obolibrary.org/obo/GAZ_00032660"/>
        <obo:IAO_0000115>A suburb of Windhoek.</obo:IAO_0000115>
        <oboInOwl:hasOBONamespace>GAZ</oboInOwl:hasOBONamespace>
        <oboInOwl:id>GAZ:00239475</oboInOwl:id>
        <rdfs:label>Windhoek West</rdfs:label>
    </owl:NamedIndividual>
    


    <!-- http://purl.obolibrary.org/obo/GAZ_00239476 -->

    <owl:NamedIndividual rdf:about="http://purl.obolibrary.org/obo/GAZ_00239476">
        <obo:RO_0001025 rdf:resource="http://purl.obolibrary.org/obo/GAZ_00014899"/>
        <obo:IAO_0000115>A constituency in Omaheke Region, Namibia.</obo:IAO_0000115>
        <oboInOwl:hasOBONamespace>GAZ</oboInOwl:hasOBONamespace>
        <oboInOwl:id>GAZ:00239476</oboInOwl:id>
        <rdfs:label>Kalahari Constituency</rdfs:label>
    </owl:NamedIndividual>
    


    <!-- http://purl.obolibrary.org/obo/GAZ_00239477 -->

    <owl:NamedIndividual rdf:about="http://purl.obolibrary.org/obo/GAZ_00239477">
        <obo:RO_0001025 rdf:resource="http://purl.obolibrary.org/obo/GAZ_00032716"/>
        <obo:IAO_0000115>A river.</obo:IAO_0000115>
        <oboInOwl:hasOBONamespace>GAZ</oboInOwl:hasOBONamespace>
        <oboInOwl:id>GAZ:00239477</oboInOwl:id>
        <rdfs:label>Omatjenne River</rdfs:label>
    </owl:NamedIndividual>
    


    <!-- http://purl.obolibrary.org/obo/GAZ_00239478 -->

    <owl:NamedIndividual rdf:about="http://purl.obolibrary.org/obo/GAZ_00239478">
        <obo:RO_0001025 rdf:resource="http://purl.obolibrary.org/obo/GAZ_00239477"/>
        <obo:IAO_0000115>A dam. Located 15km northwest of Otjiwarongo, it dams the Omatjenne River. Completed 1933.</obo:IAO_0000115>
        <oboInOwl:hasOBONamespace>GAZ</oboInOwl:hasOBONamespace>
        <oboInOwl:id>GAZ:00239478</oboInOwl:id>
        <rdfs:label>Omatjenne Dam</rdfs:label>
    </owl:NamedIndividual>
    


    <!-- http://purl.obolibrary.org/obo/GAZ_00239479 -->

    <owl:NamedIndividual rdf:about="http://purl.obolibrary.org/obo/GAZ_00239479">
        <obo:RO_0001025 rdf:resource="http://purl.obolibrary.org/obo/GAZ_00014907"/>
        <obo:IAO_0000115>A constituency in the Otjozondjupa Region of Namibia.</obo:IAO_0000115>
        <oboInOwl:hasOBONamespace>GAZ</oboInOwl:hasOBONamespace>
        <oboInOwl:id>GAZ:00239479</oboInOwl:id>
        <rdfs:label>Tsumkwe Constituency</rdfs:label>
    </owl:NamedIndividual>
    


    <!-- http://purl.obolibrary.org/obo/GAZ_00239480 -->

    <owl:NamedIndividual rdf:about="http://purl.obolibrary.org/obo/GAZ_00239480">
        <obo:RO_0001025 rdf:resource="http://purl.obolibrary.org/obo/GAZ_00239479"/>
        <obo:IAO_0000115>A protected area.</obo:IAO_0000115>
        <oboInOwl:hasOBONamespace>GAZ</oboInOwl:hasOBONamespace>
        <oboInOwl:id>GAZ:00239480</oboInOwl:id>
        <rdfs:label>Khaudum Game Reserve</rdfs:label>
    </owl:NamedIndividual>
    


    <!-- http://purl.obolibrary.org/obo/GAZ_00239481 -->

    <owl:NamedIndividual rdf:about="http://purl.obolibrary.org/obo/GAZ_00239481">
        <rdf:type rdf:resource="http://purl.obolibrary.org/obo/ENVO_00000305"/>
        <obo:RO_0001025 rdf:resource="http://purl.obolibrary.org/obo/GAZ_00014906"/>
        <obo:IAO_0000115>A cape in the South Atlantic on the coast of Namibia.</obo:IAO_0000115>
        <oboInOwl:hasOBONamespace>GAZ</oboInOwl:hasOBONamespace>
        <oboInOwl:id>GAZ:00239481</oboInOwl:id>
        <rdfs:label>Cape Cross</rdfs:label>
    </owl:NamedIndividual>
    


    <!-- http://purl.obolibrary.org/obo/GAZ_00239482 -->

    <owl:NamedIndividual rdf:about="http://purl.obolibrary.org/obo/GAZ_00239482">
        <obo:RO_0001025 rdf:resource="http://purl.obolibrary.org/obo/GAZ_00014901"/>
        <obo:IAO_0000115>A lake in Northern Namibia. Located 20 km outside of Tsumeb. A dolomite sink hole on the Waterberg Plateau, ESE of Etosha Pan.</obo:IAO_0000115>
        <oboInOwl:hasOBONamespace>GAZ</oboInOwl:hasOBONamespace>
        <oboInOwl:id>GAZ:00239482</oboInOwl:id>
        <rdfs:label>Otjikoto Lake</rdfs:label>
    </owl:NamedIndividual>
    


    <!-- http://purl.obolibrary.org/obo/GAZ_00239483 -->

    <owl:NamedIndividual rdf:about="http://purl.obolibrary.org/obo/GAZ_00239483">
        <obo:RO_0001025 rdf:resource="http://purl.obolibrary.org/obo/GAZ_00014901"/>
        <obo:IAO_0000115>A lake in northern Namibia. Located 32 km north of Tsumeb. A dolomite sinkhole.</obo:IAO_0000115>
        <oboInOwl:hasOBONamespace>GAZ</oboInOwl:hasOBONamespace>
        <oboInOwl:id>GAZ:00239483</oboInOwl:id>
        <rdfs:label>Lake Guinas</rdfs:label>
    </owl:NamedIndividual>
    


    <!-- http://purl.obolibrary.org/obo/GAZ_00239484 -->

    <owl:NamedIndividual rdf:about="http://purl.obolibrary.org/obo/GAZ_00239484">
        <obo:RO_0001025 rdf:resource="http://purl.obolibrary.org/obo/GAZ_00014897"/>
        <obo:IAO_0000115>A protected area.</obo:IAO_0000115>
        <oboInOwl:hasOBONamespace>GAZ</oboInOwl:hasOBONamespace>
        <oboInOwl:id>GAZ:00239484</oboInOwl:id>
        <rdfs:label>Kaokoland Nature Reserve</rdfs:label>
    </owl:NamedIndividual>
    


    <!-- http://purl.obolibrary.org/obo/GAZ_00239485 -->

    <owl:NamedIndividual rdf:about="http://purl.obolibrary.org/obo/GAZ_00239485">
        <obo:RO_0001025 rdf:resource="http://purl.obolibrary.org/obo/GAZ_00076647"/>
        <obo:IAO_0000115>A massif in central Namibia, forming the easternmost part of the Namib-Naukluft National Park.</obo:IAO_0000115>
        <oboInOwl:hasOBONamespace>GAZ</oboInOwl:hasOBONamespace>
        <oboInOwl:id>GAZ:00239485</oboInOwl:id>
        <rdfs:label>Naukluft Mountains</rdfs:label>
    </owl:NamedIndividual>
    


    <!-- http://purl.obolibrary.org/obo/GAZ_00239487 -->

    <owl:NamedIndividual rdf:about="http://purl.obolibrary.org/obo/GAZ_00239487">
        <obo:IAO_0000115>A dam in Khomas Region, Namibia. Located 38k m southwest of Windhoek, it dams the Kuiseb River. Completed 1972.</obo:IAO_0000115>
        <oboInOwl:hasOBONamespace>GAZ</oboInOwl:hasOBONamespace>
        <oboInOwl:id>GAZ:00239487</oboInOwl:id>
        <rdfs:label>Friedenau Dam</rdfs:label>
    </owl:NamedIndividual>
    


    <!-- http://purl.obolibrary.org/obo/GAZ_00239488 -->

    <owl:NamedIndividual rdf:about="http://purl.obolibrary.org/obo/GAZ_00239488">
        <obo:RO_0001025 rdf:resource="http://purl.obolibrary.org/obo/GAZ_00014900"/>
        <obo:IAO_0000115>A river.</obo:IAO_0000115>
        <oboInOwl:hasOBONamespace>GAZ</oboInOwl:hasOBONamespace>
        <oboInOwl:id>GAZ:00239488</oboInOwl:id>
        <rdfs:label>Satco River</rdfs:label>
    </owl:NamedIndividual>
    


    <!-- http://purl.obolibrary.org/obo/GAZ_00239489 -->

    <owl:NamedIndividual rdf:about="http://purl.obolibrary.org/obo/GAZ_00239489">
        <obo:RO_0001025 rdf:resource="http://purl.obolibrary.org/obo/GAZ_00239488"/>
        <obo:IAO_0000115>A dam outside of Karasburg, Karas Region, Namibia. Located 7 km west of Karas, it dams the Satco River. Completed 1959.</obo:IAO_0000115>
        <oboInOwl:hasOBONamespace>GAZ</oboInOwl:hasOBONamespace>
        <oboInOwl:id>GAZ:00239489</oboInOwl:id>
        <rdfs:label>Bondels Dam</rdfs:label>
    </owl:NamedIndividual>
    


    <!-- http://purl.obolibrary.org/obo/GAZ_00239490 -->

    <owl:NamedIndividual rdf:about="http://purl.obolibrary.org/obo/GAZ_00239490">
        <obo:RO_0001025 rdf:resource="http://purl.obolibrary.org/obo/GAZ_00014900"/>
        <obo:IAO_0000115>A river. A tributary of the Fish River.</obo:IAO_0000115>
        <oboInOwl:hasOBONamespace>GAZ</oboInOwl:hasOBONamespace>
        <oboInOwl:id>GAZ:00239490</oboInOwl:id>
        <rdfs:label>Lowen River</rdfs:label>
    </owl:NamedIndividual>
    


    <!-- http://purl.obolibrary.org/obo/GAZ_00239491 -->

    <owl:NamedIndividual rdf:about="http://purl.obolibrary.org/obo/GAZ_00239491">
        <obo:RO_0001025 rdf:resource="http://purl.obolibrary.org/obo/GAZ_00239490"/>
        <obo:IAO_0000115>A dam outside of Keetmanshoop, Karas Region, Namibia. Impounds Naute Reservoir. Completed 1972-09.</obo:IAO_0000115>
        <oboInOwl:hasOBONamespace>GAZ</oboInOwl:hasOBONamespace>
        <oboInOwl:id>GAZ:00239491</oboInOwl:id>
        <rdfs:label>Naute Dam</rdfs:label>
    </owl:NamedIndividual>
    


    <!-- http://purl.obolibrary.org/obo/GAZ_00239492 -->

    <owl:NamedIndividual rdf:about="http://purl.obolibrary.org/obo/GAZ_00239492">
        <obo:RO_0001025 rdf:resource="http://purl.obolibrary.org/obo/GAZ_00014908"/>
        <obo:IAO_0000115>A river.</obo:IAO_0000115>
        <oboInOwl:hasOBONamespace>GAZ</oboInOwl:hasOBONamespace>
        <oboInOwl:id>GAZ:00239492</oboInOwl:id>
        <rdfs:label>Oanob River</rdfs:label>
    </owl:NamedIndividual>
    


    <!-- http://purl.obolibrary.org/obo/GAZ_00239493 -->

    <owl:NamedIndividual rdf:about="http://purl.obolibrary.org/obo/GAZ_00239493">
        <obo:RO_0001025 rdf:resource="http://purl.obolibrary.org/obo/GAZ_00239492"/>
        <obo:IAO_0000115>A dam outside of Rehoboth, Hardap Region, Namibia. Located 7 km outside of Rehoboth, it dams the Oanob River.</obo:IAO_0000115>
        <oboInOwl:hasOBONamespace>GAZ</oboInOwl:hasOBONamespace>
        <oboInOwl:id>GAZ:00239493</oboInOwl:id>
        <rdfs:label>Oanob Dam</rdfs:label>
    </owl:NamedIndividual>
    


    <!-- http://purl.obolibrary.org/obo/GAZ_00239494 -->

    <owl:NamedIndividual rdf:about="http://purl.obolibrary.org/obo/GAZ_00239494">
        <obo:RO_0001025 rdf:resource="http://purl.obolibrary.org/obo/GAZ_00014897"/>
        <obo:IAO_0000115>A hydroelectric dam of the Cunene River in Namibia.</obo:IAO_0000115>
        <oboInOwl:hasOBONamespace>GAZ</oboInOwl:hasOBONamespace>
        <oboInOwl:id>GAZ:00239494</oboInOwl:id>
        <rdfs:label>Ruacana Dam</rdfs:label>
    </owl:NamedIndividual>
    


    <!-- http://purl.obolibrary.org/obo/GAZ_00239495 -->

    <owl:NamedIndividual rdf:about="http://purl.obolibrary.org/obo/GAZ_00239495">
        <obo:RO_0001025 rdf:resource="http://purl.obolibrary.org/obo/GAZ_00014907"/>
        <obo:RO_0001025 rdf:resource="http://purl.obolibrary.org/obo/GAZ_00239439"/>
        <obo:IAO_0000115>A dam outside of Okahandja, Otjozondjupa Region, Namibia.</obo:IAO_0000115>
        <oboInOwl:hasOBONamespace>GAZ</oboInOwl:hasOBONamespace>
        <oboInOwl:id>GAZ:00239495</oboInOwl:id>
        <rdfs:label>Swakoppoort Dam</rdfs:label>
    </owl:NamedIndividual>
    


    <!-- http://purl.obolibrary.org/obo/GAZ_00239496 -->

    <owl:NamedIndividual rdf:about="http://purl.obolibrary.org/obo/GAZ_00239496">
        <obo:RO_0001025 rdf:resource="http://purl.obolibrary.org/obo/GAZ_00252426"/>
        <obo:IAO_0000115>A dam. Impounds Von Bach Reservoir. Constructed 1968-1970.</obo:IAO_0000115>
        <oboInOwl:hasOBONamespace>GAZ</oboInOwl:hasOBONamespace>
        <oboInOwl:id>GAZ:00239496</oboInOwl:id>
        <rdfs:label>Sartorius Von Bach Dam</rdfs:label>
    </owl:NamedIndividual>
    


    <!-- http://purl.obolibrary.org/obo/GAZ_00239497 -->

    <owl:NamedIndividual rdf:about="http://purl.obolibrary.org/obo/GAZ_00239497">
        <obo:RO_0001025 rdf:resource="http://purl.obolibrary.org/obo/GAZ_00014898"/>
        <obo:IAO_0000115>A protected area. Located near Windhoek, Namibia.</obo:IAO_0000115>
        <oboInOwl:hasOBONamespace>GAZ</oboInOwl:hasOBONamespace>
        <oboInOwl:id>GAZ:00239497</oboInOwl:id>
        <rdfs:label>Daan Viljoen Game Reserve</rdfs:label>
    </owl:NamedIndividual>
    


    <!-- http://purl.obolibrary.org/obo/GAZ_00239498 -->

    <owl:NamedIndividual rdf:about="http://purl.obolibrary.org/obo/GAZ_00239498">
        <obo:RO_0001025 rdf:resource="http://purl.obolibrary.org/obo/GAZ_00014906"/>
        <obo:IAO_0000115>An ephemeral river crossing the Erongo region of central Namibia. The Khan has its origin near the settlement of Otjisemba north-west of Okahandja. From there the river course passes westwards to the town of Usakos, and further in south-western direction through the Namib desert. It has its confluence with Swakop River 40 km east of Swakopmund.</obo:IAO_0000115>
        <oboInOwl:hasOBONamespace>GAZ</oboInOwl:hasOBONamespace>
        <oboInOwl:id>GAZ:00239498</oboInOwl:id>
        <rdfs:label>Khan River</rdfs:label>
    </owl:NamedIndividual>
    


    <!-- http://purl.obolibrary.org/obo/GAZ_00239499 -->

    <owl:NamedIndividual rdf:about="http://purl.obolibrary.org/obo/GAZ_00239499">
        <obo:RO_0001025 rdf:resource="http://purl.obolibrary.org/obo/GAZ_00032658"/>
        <obo:IAO_0000115>A bay.</obo:IAO_0000115>
        <oboInOwl:hasOBONamespace>GAZ</oboInOwl:hasOBONamespace>
        <oboInOwl:id>GAZ:00239499</oboInOwl:id>
        <rdfs:label>Spencer Bay</rdfs:label>
    </owl:NamedIndividual>
    


    <!-- http://purl.obolibrary.org/obo/GAZ_00239500 -->

    <owl:NamedIndividual rdf:about="http://purl.obolibrary.org/obo/GAZ_00239500">
        <obo:RO_0001025 rdf:resource="http://purl.obolibrary.org/obo/GAZ_00239502"/>
        <obo:IAO_0000115>An island.</obo:IAO_0000115>
        <oboInOwl:hasOBONamespace>GAZ</oboInOwl:hasOBONamespace>
        <oboInOwl:id>GAZ:00239500</oboInOwl:id>
        <rdfs:label>Ichaboe Island</rdfs:label>
    </owl:NamedIndividual>
    


    <!-- http://purl.obolibrary.org/obo/GAZ_00239501 -->

    <owl:NamedIndividual rdf:about="http://purl.obolibrary.org/obo/GAZ_00239501">
        <obo:RO_0001025 rdf:resource="http://purl.obolibrary.org/obo/GAZ_00014908"/>
        <obo:IAO_0000115>A protected area. Establishd 1992.</obo:IAO_0000115>
        <oboInOwl:hasOBONamespace>GAZ</oboInOwl:hasOBONamespace>
        <oboInOwl:id>GAZ:00239501</oboInOwl:id>
        <rdfs:label>NamibRand Nature Reserve</rdfs:label>
    </owl:NamedIndividual>
    


    <!-- http://purl.obolibrary.org/obo/GAZ_00239502 -->

    <owl:NamedIndividual rdf:about="http://purl.obolibrary.org/obo/GAZ_00239502">
        <obo:RO_0001025 rdf:resource="http://purl.obolibrary.org/obo/GAZ_00014900"/>
        <obo:IAO_0000115>A group of islands and rocks situated along a stretch of 355 km along the coastline of Namibia.</obo:IAO_0000115>
        <oboInOwl:hasOBONamespace>GAZ</oboInOwl:hasOBONamespace>
        <oboInOwl:id>GAZ:00239502</oboInOwl:id>
        <rdfs:label>Penguin Islands</rdfs:label>
    </owl:NamedIndividual>
    


    <!-- http://purl.obolibrary.org/obo/GAZ_00239503 -->

    <owl:NamedIndividual rdf:about="http://purl.obolibrary.org/obo/GAZ_00239503">
        <obo:RO_0001025 rdf:resource="http://purl.obolibrary.org/obo/GAZ_00014900"/>
        <obo:IAO_0000115>A bay.</obo:IAO_0000115>
        <oboInOwl:hasOBONamespace>GAZ</oboInOwl:hasOBONamespace>
        <oboInOwl:id>GAZ:00239503</oboInOwl:id>
        <rdfs:label>Baker&apos;s Bay</rdfs:label>
    </owl:NamedIndividual>
    


    <!-- http://purl.obolibrary.org/obo/GAZ_00239504 -->

    <owl:NamedIndividual rdf:about="http://purl.obolibrary.org/obo/GAZ_00239504">
        <obo:RO_0001025 rdf:resource="http://purl.obolibrary.org/obo/GAZ_00239502"/>
        <obo:RO_0001025 rdf:resource="http://purl.obolibrary.org/obo/GAZ_00239503"/>
        <obo:IAO_0000115>Islands.</obo:IAO_0000115>
        <oboInOwl:hasOBONamespace>GAZ</oboInOwl:hasOBONamespace>
        <oboInOwl:id>GAZ:00239504</oboInOwl:id>
        <rdfs:label>Little Roastbeef Islets</rdfs:label>
    </owl:NamedIndividual>
    


    <!-- http://purl.obolibrary.org/obo/GAZ_00239505 -->

    <owl:NamedIndividual rdf:about="http://purl.obolibrary.org/obo/GAZ_00239505">
        <obo:RO_0001025 rdf:resource="http://purl.obolibrary.org/obo/GAZ_00239502"/>
        <obo:IAO_0000115>An island.</obo:IAO_0000115>
        <oboInOwl:hasOBONamespace>GAZ</oboInOwl:hasOBONamespace>
        <oboInOwl:id>GAZ:00239505</oboInOwl:id>
        <rdfs:label>Sparrow Hawk Island</rdfs:label>
    </owl:NamedIndividual>
    


    <!-- http://purl.obolibrary.org/obo/GAZ_00239506 -->

    <owl:NamedIndividual rdf:about="http://purl.obolibrary.org/obo/GAZ_00239506">
        <obo:RO_0001025 rdf:resource="http://purl.obolibrary.org/obo/GAZ_00051195"/>
        <obo:IAO_0000115>An island.</obo:IAO_0000115>
        <oboInOwl:hasOBONamespace>GAZ</oboInOwl:hasOBONamespace>
        <oboInOwl:id>GAZ:00239506</oboInOwl:id>
        <rdfs:label>Logan&apos;s Island</rdfs:label>
    </owl:NamedIndividual>
    


    <!-- http://purl.obolibrary.org/obo/GAZ_00239507 -->

    <owl:NamedIndividual rdf:about="http://purl.obolibrary.org/obo/GAZ_00239507">
        <obo:RO_0001025 rdf:resource="http://purl.obolibrary.org/obo/GAZ_00239502"/>
        <obo:IAO_0000115>An island.</obo:IAO_0000115>
        <oboInOwl:hasOBONamespace>GAZ</oboInOwl:hasOBONamespace>
        <oboInOwl:id>GAZ:00239507</oboInOwl:id>
        <rdfs:label>South Island</rdfs:label>
    </owl:NamedIndividual>
    


    <!-- http://purl.obolibrary.org/obo/GAZ_00239508 -->

    <owl:NamedIndividual rdf:about="http://purl.obolibrary.org/obo/GAZ_00239508">
        <obo:RO_0001025 rdf:resource="http://purl.obolibrary.org/obo/GAZ_00239502"/>
        <obo:IAO_0000115>Rocks.</obo:IAO_0000115>
        <oboInOwl:hasOBONamespace>GAZ</oboInOwl:hasOBONamespace>
        <oboInOwl:id>GAZ:00239508</oboInOwl:id>
        <rdfs:label>Staple Rock</rdfs:label>
    </owl:NamedIndividual>
    


    <!-- http://purl.obolibrary.org/obo/GAZ_00239509 -->

    <owl:NamedIndividual rdf:about="http://purl.obolibrary.org/obo/GAZ_00239509">
        <obo:RO_0001025 rdf:resource="http://purl.obolibrary.org/obo/GAZ_00239502"/>
        <obo:IAO_0000115>Offshore rocks.</obo:IAO_0000115>
        <oboInOwl:hasOBONamespace>GAZ</oboInOwl:hasOBONamespace>
        <oboInOwl:id>GAZ:00239509</oboInOwl:id>
        <rdfs:label>Marshall Reef</rdfs:label>
    </owl:NamedIndividual>
    


    <!-- http://purl.obolibrary.org/obo/GAZ_00239510 -->

    <owl:NamedIndividual rdf:about="http://purl.obolibrary.org/obo/GAZ_00239510">
        <obo:RO_0001025 rdf:resource="http://purl.obolibrary.org/obo/GAZ_00239502"/>
        <obo:IAO_0000115>Offshore rocks.</obo:IAO_0000115>
        <oboInOwl:hasOBONamespace>GAZ</oboInOwl:hasOBONamespace>
        <oboInOwl:id>GAZ:00239510</oboInOwl:id>
        <rdfs:label>Boat Bay Rocks</rdfs:label>
    </owl:NamedIndividual>
    


    <!-- http://purl.obolibrary.org/obo/GAZ_00239511 -->

    <owl:NamedIndividual rdf:about="http://purl.obolibrary.org/obo/GAZ_00239511">
        <obo:RO_0001025 rdf:resource="http://purl.obolibrary.org/obo/GAZ_00239502"/>
        <obo:IAO_0000115>Offshore rock.</obo:IAO_0000115>
        <oboInOwl:hasOBONamespace>GAZ</oboInOwl:hasOBONamespace>
        <oboInOwl:id>GAZ:00239511</oboInOwl:id>
        <rdfs:label>Black Sophie Rock</rdfs:label>
    </owl:NamedIndividual>
    


    <!-- http://purl.obolibrary.org/obo/GAZ_00239512 -->

    <owl:NamedIndividual rdf:about="http://purl.obolibrary.org/obo/GAZ_00239512">
        <obo:IAO_0000115>A meteorite crater, located within the Namibian section of the Namib Desert. Age: Pliocene.</obo:IAO_0000115>
        <oboInOwl:hasOBONamespace>GAZ</oboInOwl:hasOBONamespace>
        <oboInOwl:id>GAZ:00239512</oboInOwl:id>
        <rdfs:label>Roter Kamm Crater</rdfs:label>
    </owl:NamedIndividual>
    


    <!-- http://purl.obolibrary.org/obo/GAZ_00239513 -->

    <owl:NamedIndividual rdf:about="http://purl.obolibrary.org/obo/GAZ_00239513">
        <obo:RO_0001025 rdf:resource="http://purl.obolibrary.org/obo/GAZ_00014900"/>
        <obo:IAO_0000115>A bay.</obo:IAO_0000115>
        <oboInOwl:hasOBONamespace>GAZ</oboInOwl:hasOBONamespace>
        <oboInOwl:id>GAZ:00239513</oboInOwl:id>
        <rdfs:label>Elizabeth Bay</rdfs:label>
    </owl:NamedIndividual>
    


    <!-- http://purl.obolibrary.org/obo/GAZ_00239514 -->

    <owl:NamedIndividual rdf:about="http://purl.obolibrary.org/obo/GAZ_00239514">
        <obo:RO_0001025 rdf:resource="http://purl.obolibrary.org/obo/GAZ_00014900"/>
        <obo:IAO_0000115>A bay.</obo:IAO_0000115>
        <oboInOwl:hasOBONamespace>GAZ</oboInOwl:hasOBONamespace>
        <oboInOwl:id>GAZ:00239514</oboInOwl:id>
        <rdfs:label>Shearwater Bay</rdfs:label>
    </owl:NamedIndividual>
    


    <!-- http://purl.obolibrary.org/obo/GAZ_00239515 -->

    <owl:NamedIndividual rdf:about="http://purl.obolibrary.org/obo/GAZ_00239515">
        <obo:RO_0001025 rdf:resource="http://purl.obolibrary.org/obo/GAZ_00014906"/>
        <obo:IAO_0000115>An intermittent river. Discharges to the Atlantic Ocean.</obo:IAO_0000115>
        <oboInOwl:hasOBONamespace>GAZ</oboInOwl:hasOBONamespace>
        <oboInOwl:id>GAZ:00239515</oboInOwl:id>
        <rdfs:label>Ugab River</rdfs:label>
    </owl:NamedIndividual>
    


    <!-- http://purl.obolibrary.org/obo/GAZ_00239516 -->

    <owl:NamedIndividual rdf:about="http://purl.obolibrary.org/obo/GAZ_00239516">
        <obo:RO_0001025 rdf:resource="http://purl.obolibrary.org/obo/GAZ_00076647"/>
        <obo:IAO_0000115>A clay pan in the central Namib Desert, lying within the Namib-Naukluft National Park, Namibia. Fed by the Tsauchab River.</obo:IAO_0000115>
        <oboInOwl:hasOBONamespace>GAZ</oboInOwl:hasOBONamespace>
        <oboInOwl:id>GAZ:00239516</oboInOwl:id>
        <rdfs:label>Sossusvlei Pan</rdfs:label>
    </owl:NamedIndividual>
    


    <!-- http://purl.obolibrary.org/obo/GAZ_00239517 -->

    <owl:NamedIndividual rdf:about="http://purl.obolibrary.org/obo/GAZ_00239517">
        <obo:RO_0001025 rdf:resource="http://purl.obolibrary.org/obo/GAZ_00014908"/>
        <obo:IAO_0000115>A canyon.</obo:IAO_0000115>
        <oboInOwl:hasOBONamespace>GAZ</oboInOwl:hasOBONamespace>
        <oboInOwl:id>GAZ:00239517</oboInOwl:id>
        <rdfs:label>Sesriem Canyon</rdfs:label>
    </owl:NamedIndividual>
    


    <!-- http://purl.obolibrary.org/obo/GAZ_00239519 -->

    <owl:NamedIndividual rdf:about="http://purl.obolibrary.org/obo/GAZ_00239519">
        <obo:RO_0001025 rdf:resource="http://purl.obolibrary.org/obo/GAZ_00076647"/>
        <obo:IAO_0000115>A clay pan located near the salt pan of Sossusvlei, inside the Namib-Naukluft Park in Namibia.</obo:IAO_0000115>
        <oboInOwl:hasOBONamespace>GAZ</oboInOwl:hasOBONamespace>
        <oboInOwl:id>GAZ:00239519</oboInOwl:id>
        <rdfs:label>Dead Vlei</rdfs:label>
    </owl:NamedIndividual>
    


    <!-- http://purl.obolibrary.org/obo/GAZ_00239520 -->

    <owl:NamedIndividual rdf:about="http://purl.obolibrary.org/obo/GAZ_00239520">
        <obo:RO_0001025 rdf:resource="http://purl.obolibrary.org/obo/GAZ_00076647"/>
        <obo:IAO_0000115>A clay pan.</obo:IAO_0000115>
        <oboInOwl:hasOBONamespace>GAZ</oboInOwl:hasOBONamespace>
        <oboInOwl:id>GAZ:00239520</oboInOwl:id>
        <rdfs:label>Hidden Vlei</rdfs:label>
    </owl:NamedIndividual>
    


    <!-- http://purl.obolibrary.org/obo/GAZ_00239521 -->

    <owl:NamedIndividual rdf:about="http://purl.obolibrary.org/obo/GAZ_00239521">
        <obo:IAO_0000115>A group of bald granite peaks located between Usakos and Swakopmund in the Namib Desert.</obo:IAO_0000115>
        <oboInOwl:hasOBONamespace>GAZ</oboInOwl:hasOBONamespace>
        <oboInOwl:id>GAZ:00239521</oboInOwl:id>
        <rdfs:label>Spitzkoppe</rdfs:label>
    </owl:NamedIndividual>
    


    <!-- http://purl.obolibrary.org/obo/GAZ_00239522 -->

    <owl:NamedIndividual rdf:about="http://purl.obolibrary.org/obo/GAZ_00239522">
        <obo:RO_0001025 rdf:resource="http://purl.obolibrary.org/obo/GAZ_00239481"/>
        <obo:IAO_0000115>A protected area.</obo:IAO_0000115>
        <oboInOwl:hasOBONamespace>GAZ</oboInOwl:hasOBONamespace>
        <oboInOwl:id>GAZ:00239522</oboInOwl:id>
        <rdfs:label>Cape Cross Reserve</rdfs:label>
    </owl:NamedIndividual>
    


    <!-- http://purl.obolibrary.org/obo/GAZ_00239523 -->

    <owl:NamedIndividual rdf:about="http://purl.obolibrary.org/obo/GAZ_00239523">
        <obo:IAO_0000115>A desert research station in the Namib Desert in Namibia. The station is approximately 85 km SE of Walvis Bay and 232 km SW of Windhoek. It is located at the northern bank of the Kuiseb River.</obo:IAO_0000115>
        <oboInOwl:hasOBONamespace>GAZ</oboInOwl:hasOBONamespace>
        <oboInOwl:id>GAZ:00239523</oboInOwl:id>
        <rdfs:label>Gobabeb</rdfs:label>
    </owl:NamedIndividual>
    


    <!-- http://purl.obolibrary.org/obo/GAZ_00239524 -->

    <owl:NamedIndividual rdf:about="http://purl.obolibrary.org/obo/GAZ_00239524">
        <obo:RO_0001025 rdf:resource="http://purl.obolibrary.org/obo/GAZ_00014900"/>
        <obo:RO_0001025 rdf:resource="http://purl.obolibrary.org/obo/GAZ_00076641"/>
        <obo:IAO_0000115>Sulfurous hot springs.</obo:IAO_0000115>
        <oboInOwl:hasOBONamespace>GAZ</oboInOwl:hasOBONamespace>
        <oboInOwl:id>GAZ:00239524</oboInOwl:id>
        <rdfs:label>Ai-Ais Hot Springs</rdfs:label>
    </owl:NamedIndividual>
    


    <!-- http://purl.obolibrary.org/obo/GAZ_00239525 -->

    <owl:NamedIndividual rdf:about="http://purl.obolibrary.org/obo/GAZ_00239525">
        <obo:RO_0001025 rdf:resource="http://purl.obolibrary.org/obo/GAZ_00014907"/>
        <obo:IAO_0000115>Hot springs.</obo:IAO_0000115>
        <oboInOwl:hasOBONamespace>GAZ</oboInOwl:hasOBONamespace>
        <oboInOwl:id>GAZ:00239525</oboInOwl:id>
        <rdfs:label>Warme Quellen Gross Barmen</rdfs:label>
    </owl:NamedIndividual>
    


    <!-- http://purl.obolibrary.org/obo/GAZ_00239526 -->

    <owl:NamedIndividual rdf:about="http://purl.obolibrary.org/obo/GAZ_00239526">
        <obo:RO_0001025 rdf:resource="http://purl.obolibrary.org/obo/GAZ_00014908"/>
        <obo:IAO_0000115>A protected area.</obo:IAO_0000115>
        <oboInOwl:hasOBONamespace>GAZ</oboInOwl:hasOBONamespace>
        <oboInOwl:id>GAZ:00239526</oboInOwl:id>
        <rdfs:label>Hardap Recreation Resort</rdfs:label>
    </owl:NamedIndividual>
    


    <!-- http://purl.obolibrary.org/obo/GAZ_00239527 -->

    <owl:NamedIndividual rdf:about="http://purl.obolibrary.org/obo/GAZ_00239527">
        <obo:RO_0001025 rdf:resource="http://purl.obolibrary.org/obo/GAZ_00014900"/>
        <obo:IAO_0000115>A protected area.</obo:IAO_0000115>
        <oboInOwl:hasOBONamespace>GAZ</oboInOwl:hasOBONamespace>
        <oboInOwl:id>GAZ:00239527</oboInOwl:id>
        <rdfs:label>Nationales Erholungsgebiet Diamantenkuste</rdfs:label>
    </owl:NamedIndividual>
    


    <!-- http://purl.obolibrary.org/obo/GAZ_00239528 -->

    <owl:NamedIndividual rdf:about="http://purl.obolibrary.org/obo/GAZ_00239528">
        <obo:RO_0001025 rdf:resource="http://purl.obolibrary.org/obo/GAZ_00014900"/>
        <obo:IAO_0000115>A diamond mining area in south-western Namibia, in the Namib Desert. It spans the Atlantic Ocean-facing coast from Oranjemund on the border with South Africa, to around 45 miles north of Luderitz, a distance of 320 km north.</obo:IAO_0000115>
        <oboInOwl:hasOBONamespace>GAZ</oboInOwl:hasOBONamespace>
        <oboInOwl:id>GAZ:00239528</oboInOwl:id>
        <rdfs:label>Sperrgebiet</rdfs:label>
    </owl:NamedIndividual>
    


    <!-- http://purl.obolibrary.org/obo/GAZ_00239529 -->

    <owl:NamedIndividual rdf:about="http://purl.obolibrary.org/obo/GAZ_00239529">
        <obo:RO_0001025 rdf:resource="http://purl.obolibrary.org/obo/GAZ_00239528"/>
        <obo:IAO_0000115>A national partk. Established 2004.</obo:IAO_0000115>
        <oboInOwl:hasOBONamespace>GAZ</oboInOwl:hasOBONamespace>
        <oboInOwl:id>GAZ:00239529</oboInOwl:id>
        <rdfs:label>Sperrgebiet National Park</rdfs:label>
    </owl:NamedIndividual>
    


    <!-- http://purl.obolibrary.org/obo/GAZ_00239572 -->

    <owl:NamedIndividual rdf:about="http://purl.obolibrary.org/obo/GAZ_00239572">
        <obo:IAO_0000115>A reservoir. Impounded by Gariep Dam. Completed 1971.</obo:IAO_0000115>
        <oboInOwl:hasOBONamespace>GAZ</oboInOwl:hasOBONamespace>
        <oboInOwl:id>GAZ:00239572</oboInOwl:id>
        <rdfs:label>Lake Gariep</rdfs:label>
    </owl:NamedIndividual>
    


    <!-- http://purl.obolibrary.org/obo/GAZ_00239573 -->

    <owl:NamedIndividual rdf:about="http://purl.obolibrary.org/obo/GAZ_00239573">
        <obo:IAO_0000115>A dam impounding Lake Gariep. Located between the Eastern Cape to the south and the Free State to the north and about 30 km north east of Colesberg. It is situated in a gorge at the entrance to the Ruigte Valley some 5 km east of Norvalspont. Completed 1971.</obo:IAO_0000115>
        <oboInOwl:hasOBONamespace>GAZ</oboInOwl:hasOBONamespace>
        <oboInOwl:id>GAZ:00239573</oboInOwl:id>
        <rdfs:label>Gariep Dam</rdfs:label>
    </owl:NamedIndividual>
    


    <!-- http://purl.obolibrary.org/obo/GAZ_00239579 -->

    <owl:NamedIndividual rdf:about="http://purl.obolibrary.org/obo/GAZ_00239579">
        <obo:IAO_0000115>A river.</obo:IAO_0000115>
        <oboInOwl:hasOBONamespace>GAZ</oboInOwl:hasOBONamespace>
        <oboInOwl:id>GAZ:00239579</oboInOwl:id>
        <rdfs:label>Nuwejaarspruit</rdfs:label>
    </owl:NamedIndividual>
    


    <!-- http://purl.obolibrary.org/obo/GAZ_00239580 -->

    <owl:NamedIndividual rdf:about="http://purl.obolibrary.org/obo/GAZ_00239580">
        <obo:RO_0001025 rdf:resource="http://purl.obolibrary.org/obo/GAZ_00239579"/>
        <obo:IAO_0000115>A dam. Located just outside the town of Harrismith, is part of the Tugela-Vaal Water Project. Impounds Sterkfontein Dam Reservoir. Completed 1977.</obo:IAO_0000115>
        <oboInOwl:hasOBONamespace>GAZ</oboInOwl:hasOBONamespace>
        <oboInOwl:id>GAZ:00239580</oboInOwl:id>
        <rdfs:label>Sterkfontein Dam</rdfs:label>
    </owl:NamedIndividual>
    


    <!-- http://purl.obolibrary.org/obo/GAZ_00239581 -->

    <owl:NamedIndividual rdf:about="http://purl.obolibrary.org/obo/GAZ_00239581">
        <obo:RO_0001025 rdf:resource="http://purl.obolibrary.org/obo/GAZ_00239579"/>
        <obo:IAO_0000115>A reservoir. Impounded by Sterkfontein Dam. Completed 1977.</obo:IAO_0000115>
        <oboInOwl:hasOBONamespace>GAZ</oboInOwl:hasOBONamespace>
        <oboInOwl:id>GAZ:00239581</oboInOwl:id>
        <rdfs:label>Sterkfontein Dam Reservoir</rdfs:label>
    </owl:NamedIndividual>
    


    <!-- http://purl.obolibrary.org/obo/GAZ_00239591 -->

    <owl:NamedIndividual rdf:about="http://purl.obolibrary.org/obo/GAZ_00239591">
        <obo:IAO_0000115>A dam. Located on the Vaal River, downstream of Vaal Dam approximately 2 km upstream of the town of Bloemhof. Impounds Bloemhof Dam Reservoir. Completed 1970.</obo:IAO_0000115>
        <oboInOwl:hasOBONamespace>GAZ</oboInOwl:hasOBONamespace>
        <oboInOwl:id>GAZ:00239591</oboInOwl:id>
        <rdfs:label>Bloemhof Dam</rdfs:label>
    </owl:NamedIndividual>
    


    <!-- http://purl.obolibrary.org/obo/GAZ_00239592 -->

    <owl:NamedIndividual rdf:about="http://purl.obolibrary.org/obo/GAZ_00239592">
        <obo:IAO_0000115>A reservoir. Impounded by Bloemhof Dam. Completed 1970.</obo:IAO_0000115>
        <oboInOwl:hasOBONamespace>GAZ</oboInOwl:hasOBONamespace>
        <oboInOwl:id>GAZ:00239592</oboInOwl:id>
        <rdfs:label>Bloemhof Dam Reservoir</rdfs:label>
    </owl:NamedIndividual>
    


    <!-- http://purl.obolibrary.org/obo/GAZ_00239942 -->

    <owl:NamedIndividual rdf:about="http://purl.obolibrary.org/obo/GAZ_00239942">
        <obo:IAO_0000115>A dam.</obo:IAO_0000115>
        <oboInOwl:hasOBONamespace>GAZ</oboInOwl:hasOBONamespace>
        <oboInOwl:id>GAZ:00239942</oboInOwl:id>
        <rdfs:label>Van der Kloof Dam</rdfs:label>
    </owl:NamedIndividual>
    


    <!-- http://purl.obolibrary.org/obo/GAZ_00239943 -->

    <owl:NamedIndividual rdf:about="http://purl.obolibrary.org/obo/GAZ_00239943">
        <obo:IAO_0000115>A river that drains part of the north eastern Karoo into the Orange River above the Van der Kloof Dam.</obo:IAO_0000115>
        <oboInOwl:hasOBONamespace>GAZ</oboInOwl:hasOBONamespace>
        <oboInOwl:id>GAZ:00239943</oboInOwl:id>
        <rdfs:label>Seekoei River</rdfs:label>
    </owl:NamedIndividual>
    


    <!-- http://purl.obolibrary.org/obo/GAZ_00239944 -->

    <owl:NamedIndividual rdf:about="http://purl.obolibrary.org/obo/GAZ_00239944">
        <obo:IAO_0000115>A river. A tributary of the Orange River that rises near Hanover.</obo:IAO_0000115>
        <oboInOwl:hasOBONamespace>GAZ</oboInOwl:hasOBONamespace>
        <oboInOwl:id>GAZ:00239944</oboInOwl:id>
        <rdfs:label>Brak River</rdfs:label>
    </owl:NamedIndividual>
    


    <!-- http://purl.obolibrary.org/obo/GAZ_00239945 -->

    <owl:NamedIndividual rdf:about="http://purl.obolibrary.org/obo/GAZ_00239945">
        <obo:IAO_0000115>A river. A tributary of the Brak River that rises near Richmond.</obo:IAO_0000115>
        <oboInOwl:hasOBONamespace>GAZ</oboInOwl:hasOBONamespace>
        <oboInOwl:id>GAZ:00239945</oboInOwl:id>
        <rdfs:label>Ongers River</rdfs:label>
    </owl:NamedIndividual>
    


    <!-- http://purl.obolibrary.org/obo/GAZ_00239946 -->

    <owl:NamedIndividual rdf:about="http://purl.obolibrary.org/obo/GAZ_00239946">
        <obo:IAO_0000115>A river. A tributary of the Orange River.</obo:IAO_0000115>
        <oboInOwl:hasOBONamespace>GAZ</oboInOwl:hasOBONamespace>
        <oboInOwl:id>GAZ:00239946</oboInOwl:id>
        <rdfs:label>Hartebeest River</rdfs:label>
    </owl:NamedIndividual>
    


    <!-- http://purl.obolibrary.org/obo/GAZ_00240186 -->

    <owl:NamedIndividual rdf:about="http://purl.obolibrary.org/obo/GAZ_00240186">
        <obo:IAO_0000115>A dam. Constructed 1973.</obo:IAO_0000115>
        <oboInOwl:hasOBONamespace>GAZ</oboInOwl:hasOBONamespace>
        <oboInOwl:id>GAZ:00240186</oboInOwl:id>
        <rdfs:label>Welbedacht Dam</rdfs:label>
    </owl:NamedIndividual>
    


    <!-- http://purl.obolibrary.org/obo/GAZ_00240191 -->

    <owl:NamedIndividual rdf:about="http://purl.obolibrary.org/obo/GAZ_00240191">
        <obo:IAO_0000115>A river of Free State Province.</obo:IAO_0000115>
        <oboInOwl:hasOBONamespace>GAZ</oboInOwl:hasOBONamespace>
        <oboInOwl:id>GAZ:00240191</oboInOwl:id>
        <rdfs:label>Vals River</rdfs:label>
    </owl:NamedIndividual>
    


    <!-- http://purl.obolibrary.org/obo/GAZ_00240192 -->

    <owl:NamedIndividual rdf:about="http://purl.obolibrary.org/obo/GAZ_00240192">
        <obo:IAO_0000115>A river of Free State Province.</obo:IAO_0000115>
        <oboInOwl:hasOBONamespace>GAZ</oboInOwl:hasOBONamespace>
        <oboInOwl:id>GAZ:00240192</oboInOwl:id>
        <rdfs:label>Vet River</rdfs:label>
    </owl:NamedIndividual>
    


    <!-- http://purl.obolibrary.org/obo/GAZ_00240193 -->

    <owl:NamedIndividual rdf:about="http://purl.obolibrary.org/obo/GAZ_00240193">
        <obo:IAO_0000115>A river of Free State Province.</obo:IAO_0000115>
        <oboInOwl:hasOBONamespace>GAZ</oboInOwl:hasOBONamespace>
        <oboInOwl:id>GAZ:00240193</oboInOwl:id>
        <rdfs:label>Wilge River</rdfs:label>
    </owl:NamedIndividual>
    


    <!-- http://purl.obolibrary.org/obo/GAZ_00240220 -->

    <owl:NamedIndividual rdf:about="http://purl.obolibrary.org/obo/GAZ_00240220">
        <obo:IAO_0000115>A dam.</obo:IAO_0000115>
        <oboInOwl:hasOBONamespace>GAZ</oboInOwl:hasOBONamespace>
        <oboInOwl:id>GAZ:00240220</oboInOwl:id>
        <rdfs:label>Newberry Dam</rdfs:label>
    </owl:NamedIndividual>
    


    <!-- http://purl.obolibrary.org/obo/GAZ_00240234 -->

    <owl:NamedIndividual rdf:about="http://purl.obolibrary.org/obo/GAZ_00240234">
        <obo:IAO_0000115>A dam.</obo:IAO_0000115>
        <oboInOwl:hasOBONamespace>GAZ</oboInOwl:hasOBONamespace>
        <oboInOwl:id>GAZ:00240234</oboInOwl:id>
        <rdfs:label>Grootdraai Dam</rdfs:label>
    </owl:NamedIndividual>
    


    <!-- http://purl.obolibrary.org/obo/GAZ_00240257 -->

    <owl:NamedIndividual rdf:about="http://purl.obolibrary.org/obo/GAZ_00240257">
        <obo:RO_0001025 rdf:resource="http://purl.obolibrary.org/obo/GAZ_00240192"/>
        <obo:IAO_0000115>A dam. Constructed 1960.</obo:IAO_0000115>
        <oboInOwl:hasOBONamespace>GAZ</oboInOwl:hasOBONamespace>
        <oboInOwl:id>GAZ:00240257</oboInOwl:id>
        <rdfs:label>Erfenis Dam</rdfs:label>
    </owl:NamedIndividual>
    


    <!-- http://purl.obolibrary.org/obo/GAZ_00240261 -->

    <owl:NamedIndividual rdf:about="http://purl.obolibrary.org/obo/GAZ_00240261">
        <obo:IAO_0000115>A dam. Constructed 1938.</obo:IAO_0000115>
        <oboInOwl:hasOBONamespace>GAZ</oboInOwl:hasOBONamespace>
        <oboInOwl:id>GAZ:00240261</oboInOwl:id>
        <rdfs:label>Kalkfontein Dam</rdfs:label>
    </owl:NamedIndividual>
    


    <!-- http://purl.obolibrary.org/obo/GAZ_00246622 -->

    <owl:NamedIndividual rdf:about="http://purl.obolibrary.org/obo/GAZ_00246622">
        <obo:IAO_0000115>A man-made lake.</obo:IAO_0000115>
        <oboInOwl:hasOBONamespace>GAZ</oboInOwl:hasOBONamespace>
        <oboInOwl:id>GAZ:00246622</oboInOwl:id>
        <rdfs:label>Chinchama Lake</rdfs:label>
    </owl:NamedIndividual>
    


    <!-- http://purl.obolibrary.org/obo/GAZ_00246623 -->

    <owl:NamedIndividual rdf:about="http://purl.obolibrary.org/obo/GAZ_00246623">
        <obo:IAO_0000115>A river. Joins the Rio Cunene at Matala.</obo:IAO_0000115>
        <oboInOwl:hasOBONamespace>GAZ</oboInOwl:hasOBONamespace>
        <oboInOwl:id>GAZ:00246623</oboInOwl:id>
        <rdfs:label>Rio Catape</rdfs:label>
    </owl:NamedIndividual>
    


    <!-- http://purl.obolibrary.org/obo/GAZ_00246625 -->

    <owl:NamedIndividual rdf:about="http://purl.obolibrary.org/obo/GAZ_00246625">
        <obo:IAO_0000115>A river. It joins the Rio Cunene just below Xangongo.</obo:IAO_0000115>
        <oboInOwl:hasOBONamespace>GAZ</oboInOwl:hasOBONamespace>
        <oboInOwl:id>GAZ:00246625</oboInOwl:id>
        <rdfs:label>Rio Caculuvar</rdfs:label>
    </owl:NamedIndividual>
    


    <!-- http://purl.obolibrary.org/obo/GAZ_00246864 -->

    <owl:NamedIndividual rdf:about="http://purl.obolibrary.org/obo/GAZ_00246864">
        <rdf:type rdf:resource="http://purl.obolibrary.org/obo/ENVO_00000309"/>
        <obo:RO_0001025 rdf:resource="http://purl.obolibrary.org/obo/GAZ_00076291"/>
        <obo:IAO_0000115>A pan.</obo:IAO_0000115>
        <oboInOwl:hasOBONamespace>GAZ</oboInOwl:hasOBONamespace>
        <oboInOwl:id>GAZ:00246864</oboInOwl:id>
        <rdfs:label>Kgama Kgama Pan</rdfs:label>
    </owl:NamedIndividual>
    


    <!-- http://purl.obolibrary.org/obo/GAZ_00247716 -->

    <owl:NamedIndividual rdf:about="http://purl.obolibrary.org/obo/GAZ_00247716">
        <obo:IAO_0000115>A river.</obo:IAO_0000115>
        <oboInOwl:hasOBONamespace>GAZ</oboInOwl:hasOBONamespace>
        <oboInOwl:id>GAZ:00247716</oboInOwl:id>
        <rdfs:label>Mulola Chioca</rdfs:label>
    </owl:NamedIndividual>
    


    <!-- http://purl.obolibrary.org/obo/GAZ_00247717 -->

    <owl:NamedIndividual rdf:about="http://purl.obolibrary.org/obo/GAZ_00247717">
        <obo:IAO_0000115>A river.</obo:IAO_0000115>
        <oboInOwl:hasOBONamespace>GAZ</oboInOwl:hasOBONamespace>
        <oboInOwl:id>GAZ:00247717</oboInOwl:id>
        <rdfs:label>Mulola Lueque</rdfs:label>
    </owl:NamedIndividual>
    


    <!-- http://purl.obolibrary.org/obo/GAZ_00251903 -->

    <owl:NamedIndividual rdf:about="http://purl.obolibrary.org/obo/GAZ_00251903">
        <obo:IAO_0000115>A widening of the Shire River?</obo:IAO_0000115>
        <oboInOwl:hasOBONamespace>GAZ</oboInOwl:hasOBONamespace>
        <oboInOwl:id>GAZ:00251903</oboInOwl:id>
        <rdfs:label>Bangula Lagoon</rdfs:label>
    </owl:NamedIndividual>
    


    <!-- http://purl.obolibrary.org/obo/GAZ_00252406 -->

    <owl:NamedIndividual rdf:about="http://purl.obolibrary.org/obo/GAZ_00252406">
        <obo:RO_0001025 rdf:resource="http://purl.obolibrary.org/obo/GAZ_00014906"/>
        <obo:RO_0001025 rdf:resource="http://purl.obolibrary.org/obo/GAZ_00076647"/>
        <obo:IAO_0000115>A shallow lagoon lying about 80 km South of Walvis Bay. It is orientated N-S, isolated from the interior of Namibia by the sand dunes of the Namib Desert, and bounded by the Atlantic Ocean on the west. It opens to the sea centrally, between sandspits, through a mouth some 200 m across.</obo:IAO_0000115>
        <oboInOwl:hasOBONamespace>GAZ</oboInOwl:hasOBONamespace>
        <oboInOwl:id>GAZ:00252406</oboInOwl:id>
        <rdfs:label>Sandwich Harbour</rdfs:label>
    </owl:NamedIndividual>
    


    <!-- http://purl.obolibrary.org/obo/GAZ_00252407 -->

    <owl:NamedIndividual rdf:about="http://purl.obolibrary.org/obo/GAZ_00252407">
        <obo:RO_0001025 rdf:resource="http://purl.obolibrary.org/obo/GAZ_00239481"/>
        <obo:IAO_0000115>A series of small saline lagoons fed by sea water seepage and high tide washovers. Located behind a sand barrier.</obo:IAO_0000115>
        <oboInOwl:hasOBONamespace>GAZ</oboInOwl:hasOBONamespace>
        <oboInOwl:id>GAZ:00252407</oboInOwl:id>
        <rdfs:label>Cape Cross Lagoons</rdfs:label>
    </owl:NamedIndividual>
    


    <!-- http://purl.obolibrary.org/obo/GAZ_00252409 -->

    <owl:NamedIndividual rdf:about="http://purl.obolibrary.org/obo/GAZ_00252409">
        <obo:RO_0001025 rdf:resource="http://purl.obolibrary.org/obo/GAZ_00076294"/>
        <obo:IAO_0000115>A lake.</obo:IAO_0000115>
        <oboInOwl:hasOBONamespace>GAZ</oboInOwl:hasOBONamespace>
        <oboInOwl:id>GAZ:00252409</oboInOwl:id>
        <rdfs:label>Saraugxa Lediba</rdfs:label>
    </owl:NamedIndividual>
    


    <!-- http://purl.obolibrary.org/obo/GAZ_00252410 -->

    <owl:NamedIndividual rdf:about="http://purl.obolibrary.org/obo/GAZ_00252410">
        <obo:RO_0001025 rdf:resource="http://purl.obolibrary.org/obo/GAZ_00076294"/>
        <obo:IAO_0000115>A lake.</obo:IAO_0000115>
        <oboInOwl:hasOBONamespace>GAZ</oboInOwl:hasOBONamespace>
        <oboInOwl:id>GAZ:00252410</oboInOwl:id>
        <rdfs:label>Zibadianga Lediba</rdfs:label>
    </owl:NamedIndividual>
    


    <!-- http://purl.obolibrary.org/obo/GAZ_00252413 -->

    <owl:NamedIndividual rdf:about="http://purl.obolibrary.org/obo/GAZ_00252413">
        <rdf:type rdf:resource="http://purl.obolibrary.org/obo/ENVO_00000309"/>
        <obo:RO_0001025 rdf:resource="http://purl.obolibrary.org/obo/GAZ_00014897"/>
        <obo:IAO_0000115>A pan.</obo:IAO_0000115>
        <oboInOwl:hasOBONamespace>GAZ</oboInOwl:hasOBONamespace>
        <oboInOwl:id>GAZ:00252413</oboInOwl:id>
        <rdfs:label>Natukanaoka Pan</rdfs:label>
    </owl:NamedIndividual>
    


    <!-- http://purl.obolibrary.org/obo/GAZ_00252415 -->

    <owl:NamedIndividual rdf:about="http://purl.obolibrary.org/obo/GAZ_00252415">
        <rdf:type rdf:resource="http://purl.obolibrary.org/obo/ENVO_00000309"/>
        <obo:RO_0001025 rdf:resource="http://purl.obolibrary.org/obo/GAZ_00076647"/>
        <obo:IAO_0000115>A pan.</obo:IAO_0000115>
        <oboInOwl:hasOBONamespace>GAZ</oboInOwl:hasOBONamespace>
        <oboInOwl:id>GAZ:00252415</oboInOwl:id>
        <rdfs:label>Tsondabvlei Pan</rdfs:label>
    </owl:NamedIndividual>
    


    <!-- http://purl.obolibrary.org/obo/GAZ_00252416 -->

    <owl:NamedIndividual rdf:about="http://purl.obolibrary.org/obo/GAZ_00252416">
        <obo:RO_0001025 rdf:resource="http://purl.obolibrary.org/obo/GAZ_00014897"/>
        <obo:IAO_0000115>An intermittent river. Discharges to the Atlantic Ocean.</obo:IAO_0000115>
        <oboInOwl:hasOBONamespace>GAZ</oboInOwl:hasOBONamespace>
        <oboInOwl:id>GAZ:00252416</oboInOwl:id>
        <rdfs:label>Khumib River</rdfs:label>
    </owl:NamedIndividual>
    


    <!-- http://purl.obolibrary.org/obo/GAZ_00252417 -->

    <owl:NamedIndividual rdf:about="http://purl.obolibrary.org/obo/GAZ_00252417">
        <obo:RO_0001025 rdf:resource="http://purl.obolibrary.org/obo/GAZ_00014897"/>
        <obo:IAO_0000115>An intermittent river. Discharges to the Atlantic Ocean.</obo:IAO_0000115>
        <oboInOwl:hasOBONamespace>GAZ</oboInOwl:hasOBONamespace>
        <oboInOwl:id>GAZ:00252417</oboInOwl:id>
        <rdfs:label>Hoarusib River</rdfs:label>
    </owl:NamedIndividual>
    


    <!-- http://purl.obolibrary.org/obo/GAZ_00252418 -->

    <owl:NamedIndividual rdf:about="http://purl.obolibrary.org/obo/GAZ_00252418">
        <obo:IAO_0000115>An intermittent river. Discharges towards the Atlantic Ocean.</obo:IAO_0000115>
        <oboInOwl:hasOBONamespace>GAZ</oboInOwl:hasOBONamespace>
        <oboInOwl:id>GAZ:00252418</oboInOwl:id>
        <rdfs:label>Hoanib River</rdfs:label>
    </owl:NamedIndividual>
    


    <!-- http://purl.obolibrary.org/obo/GAZ_00252419 -->

    <owl:NamedIndividual rdf:about="http://purl.obolibrary.org/obo/GAZ_00252419">
        <obo:IAO_0000115>An intermittent river. Discharges to the Atlantic Ocean.</obo:IAO_0000115>
        <oboInOwl:hasOBONamespace>GAZ</oboInOwl:hasOBONamespace>
        <oboInOwl:id>GAZ:00252419</oboInOwl:id>
        <rdfs:label>Uniab River</rdfs:label>
    </owl:NamedIndividual>
    


    <!-- http://purl.obolibrary.org/obo/GAZ_00252420 -->

    <owl:NamedIndividual rdf:about="http://purl.obolibrary.org/obo/GAZ_00252420">
        <obo:IAO_0000115>An intermittent river. Discharges to the Atlantic Ocean.</obo:IAO_0000115>
        <oboInOwl:hasOBONamespace>GAZ</oboInOwl:hasOBONamespace>
        <oboInOwl:id>GAZ:00252420</oboInOwl:id>
        <rdfs:label>Huab River</rdfs:label>
    </owl:NamedIndividual>
    


    <!-- http://purl.obolibrary.org/obo/GAZ_00252422 -->

    <owl:NamedIndividual rdf:about="http://purl.obolibrary.org/obo/GAZ_00252422">
        <obo:RO_0001025 rdf:resource="http://purl.obolibrary.org/obo/GAZ_00014906"/>
        <obo:RO_0001025 rdf:resource="http://purl.obolibrary.org/obo/GAZ_00032642"/>
        <obo:IAO_0000115>An intermittent river. Discharges to the Atlantic Ocean.</obo:IAO_0000115>
        <oboInOwl:hasOBONamespace>GAZ</oboInOwl:hasOBONamespace>
        <oboInOwl:id>GAZ:00252422</oboInOwl:id>
        <rdfs:label>Omaruru River</rdfs:label>
    </owl:NamedIndividual>
    


    <!-- http://purl.obolibrary.org/obo/GAZ_00252423 -->

    <owl:NamedIndividual rdf:about="http://purl.obolibrary.org/obo/GAZ_00252423">
        <obo:RO_0001025 rdf:resource="http://purl.obolibrary.org/obo/GAZ_00239497"/>
        <obo:IAO_0000115>A dam. Impounds Augeigas Dam Reservoir.</obo:IAO_0000115>
        <oboInOwl:hasOBONamespace>GAZ</oboInOwl:hasOBONamespace>
        <oboInOwl:id>GAZ:00252423</oboInOwl:id>
        <rdfs:label>Augeigas Dam</rdfs:label>
    </owl:NamedIndividual>
    


    <!-- http://purl.obolibrary.org/obo/GAZ_00252424 -->

    <owl:NamedIndividual rdf:about="http://purl.obolibrary.org/obo/GAZ_00252424">
        <obo:RO_0001025 rdf:resource="http://purl.obolibrary.org/obo/GAZ_00239497"/>
        <obo:IAO_0000115>A reservoir. Impounded by Augeigas Dam.</obo:IAO_0000115>
        <oboInOwl:hasOBONamespace>GAZ</oboInOwl:hasOBONamespace>
        <oboInOwl:id>GAZ:00252424</oboInOwl:id>
        <rdfs:label>Augeigas Dam Reservoir</rdfs:label>
    </owl:NamedIndividual>
    


    <!-- http://purl.obolibrary.org/obo/GAZ_00252425 -->

    <owl:NamedIndividual rdf:about="http://purl.obolibrary.org/obo/GAZ_00252425">
        <obo:RO_0001025 rdf:resource="http://purl.obolibrary.org/obo/GAZ_00239490"/>
        <obo:IAO_0000115>A reservoir. Impounded by Naute Dam.</obo:IAO_0000115>
        <oboInOwl:hasOBONamespace>GAZ</oboInOwl:hasOBONamespace>
        <oboInOwl:id>GAZ:00252425</oboInOwl:id>
        <rdfs:label>Naute Reservoir</rdfs:label>
    </owl:NamedIndividual>
    


    <!-- http://purl.obolibrary.org/obo/GAZ_00252426 -->

    <owl:NamedIndividual rdf:about="http://purl.obolibrary.org/obo/GAZ_00252426">
        <obo:RO_0001025 rdf:resource="http://purl.obolibrary.org/obo/GAZ_00032718"/>
        <obo:IAO_0000115>A resort.</obo:IAO_0000115>
        <oboInOwl:hasOBONamespace>GAZ</oboInOwl:hasOBONamespace>
        <oboInOwl:id>GAZ:00252426</oboInOwl:id>
        <rdfs:label>Von Bach Recreation Resort</rdfs:label>
    </owl:NamedIndividual>
    


    <!-- http://purl.obolibrary.org/obo/GAZ_00252427 -->

    <owl:NamedIndividual rdf:about="http://purl.obolibrary.org/obo/GAZ_00252427">
        <obo:RO_0001025 rdf:resource="http://purl.obolibrary.org/obo/GAZ_00252426"/>
        <obo:IAO_0000115>A reservoir. Impounded by Sartorius Von Bach Dam.</obo:IAO_0000115>
        <oboInOwl:hasOBONamespace>GAZ</oboInOwl:hasOBONamespace>
        <oboInOwl:id>GAZ:00252427</oboInOwl:id>
        <rdfs:label>Von Bach Reservoir</rdfs:label>
    </owl:NamedIndividual>
    


    <!-- http://purl.obolibrary.org/obo/GAZ_00260937 -->

    <owl:NamedIndividual rdf:about="http://purl.obolibrary.org/obo/GAZ_00260937">
        <obo:IAO_0000115>A canal carrying water of the Luena River.</obo:IAO_0000115>
        <oboInOwl:hasOBONamespace>GAZ</oboInOwl:hasOBONamespace>
        <oboInOwl:id>GAZ:00260937</oboInOwl:id>
        <rdfs:label>Lubitanei Canal</rdfs:label>
    </owl:NamedIndividual>
    


    <!-- http://purl.obolibrary.org/obo/GAZ_00260942 -->

    <owl:NamedIndividual rdf:about="http://purl.obolibrary.org/obo/GAZ_00260942">
        <obo:IAO_0000115>A tributary which joins the Zambezi River just below Senanga on the Barotse Floodplain. It rises in Angola and drains the swampy southeastern interior of that country, including the Chiume Lakes.</obo:IAO_0000115>
        <oboInOwl:hasOBONamespace>GAZ</oboInOwl:hasOBONamespace>
        <oboInOwl:id>GAZ:00260942</oboInOwl:id>
        <rdfs:label>Lueti River</rdfs:label>
    </owl:NamedIndividual>
    


    <!-- http://purl.obolibrary.org/obo/GAZ_00260943 -->

    <owl:NamedIndividual rdf:about="http://purl.obolibrary.org/obo/GAZ_00260943">
        <obo:IAO_0000115>A tributary which joins the Zambezi River just below Senanga on the Barotse Floodplain.</obo:IAO_0000115>
        <oboInOwl:hasOBONamespace>GAZ</oboInOwl:hasOBONamespace>
        <oboInOwl:id>GAZ:00260943</oboInOwl:id>
        <rdfs:label>Lui River</rdfs:label>
    </owl:NamedIndividual>
    


    <!-- http://purl.obolibrary.org/obo/GAZ_00260944 -->

    <owl:NamedIndividual rdf:about="http://purl.obolibrary.org/obo/GAZ_00260944">
        <obo:IAO_0000115>A wetland. A floodplain along the northern border of the Caprivi Strip.</obo:IAO_0000115>
        <oboInOwl:hasOBONamespace>GAZ</oboInOwl:hasOBONamespace>
        <oboInOwl:id>GAZ:00260944</oboInOwl:id>
        <rdfs:label>Sesheke-Maramba Floodplain</rdfs:label>
    </owl:NamedIndividual>
    


    <!-- http://purl.obolibrary.org/obo/GAZ_00260974 -->

    <owl:NamedIndividual rdf:about="http://purl.obolibrary.org/obo/GAZ_00260974">
        <obo:IAO_0000115>A reservoir. Completed 1978.</obo:IAO_0000115>
        <oboInOwl:hasOBONamespace>GAZ</oboInOwl:hasOBONamespace>
        <oboInOwl:id>GAZ:00260974</oboInOwl:id>
        <rdfs:label>Lake Itezhi-Tezhi</rdfs:label>
    </owl:NamedIndividual>
    


    <!-- http://purl.obolibrary.org/obo/GAZ_00260996 -->

    <owl:NamedIndividual rdf:about="http://purl.obolibrary.org/obo/GAZ_00260996">
        <obo:RO_0001025 rdf:resource="http://purl.obolibrary.org/obo/GAZ_00016178"/>
        <obo:IAO_0000115>A river.</obo:IAO_0000115>
        <oboInOwl:hasOBONamespace>GAZ</oboInOwl:hasOBONamespace>
        <oboInOwl:id>GAZ:00260996</oboInOwl:id>
        <rdfs:label>Sebungwe River</rdfs:label>
    </owl:NamedIndividual>
    


    <!-- http://purl.obolibrary.org/obo/GAZ_00260997 -->

    <owl:NamedIndividual rdf:about="http://purl.obolibrary.org/obo/GAZ_00260997">
        <obo:RO_0001025 rdf:resource="http://purl.obolibrary.org/obo/GAZ_00016178"/>
        <obo:IAO_0000115>A river.</obo:IAO_0000115>
        <oboInOwl:hasOBONamespace>GAZ</oboInOwl:hasOBONamespace>
        <oboInOwl:id>GAZ:00260997</oboInOwl:id>
        <rdfs:label>Sengwa River</rdfs:label>
    </owl:NamedIndividual>
    


    <!-- http://purl.obolibrary.org/obo/GAZ_00260998 -->

    <owl:NamedIndividual rdf:about="http://purl.obolibrary.org/obo/GAZ_00260998">
        <obo:RO_0001025 rdf:resource="http://purl.obolibrary.org/obo/GAZ_00016178"/>
        <obo:IAO_0000115>A river.</obo:IAO_0000115>
        <oboInOwl:hasOBONamespace>GAZ</oboInOwl:hasOBONamespace>
        <oboInOwl:id>GAZ:00260998</oboInOwl:id>
        <rdfs:label>Ume River</rdfs:label>
    </owl:NamedIndividual>
    


    <!-- http://purl.obolibrary.org/obo/GAZ_00260999 -->

    <owl:NamedIndividual rdf:about="http://purl.obolibrary.org/obo/GAZ_00260999">
        <obo:RO_0001025 rdf:resource="http://purl.obolibrary.org/obo/GAZ_00016178"/>
        <obo:IAO_0000115>A river.</obo:IAO_0000115>
        <oboInOwl:hasOBONamespace>GAZ</oboInOwl:hasOBONamespace>
        <oboInOwl:id>GAZ:00260999</oboInOwl:id>
        <rdfs:label>Sanyati River</rdfs:label>
    </owl:NamedIndividual>
    


    <!-- http://purl.obolibrary.org/obo/GAZ_00261000 -->

    <owl:NamedIndividual rdf:about="http://purl.obolibrary.org/obo/GAZ_00261000">
        <obo:RO_0001025 rdf:resource="http://purl.obolibrary.org/obo/GAZ_00016178"/>
        <obo:IAO_0000115>A river.</obo:IAO_0000115>
        <oboInOwl:hasOBONamespace>GAZ</oboInOwl:hasOBONamespace>
        <oboInOwl:id>GAZ:00261000</oboInOwl:id>
        <rdfs:label>Mwenda River</rdfs:label>
    </owl:NamedIndividual>
    


    <!-- http://purl.obolibrary.org/obo/GAZ_00261001 -->

    <owl:NamedIndividual rdf:about="http://purl.obolibrary.org/obo/GAZ_00261001">
        <obo:RO_0001025 rdf:resource="http://purl.obolibrary.org/obo/GAZ_00016178"/>
        <obo:IAO_0000115>A river.</obo:IAO_0000115>
        <oboInOwl:hasOBONamespace>GAZ</oboInOwl:hasOBONamespace>
        <oboInOwl:id>GAZ:00261001</oboInOwl:id>
        <rdfs:label>Zhimu River</rdfs:label>
    </owl:NamedIndividual>
    


    <!-- http://purl.obolibrary.org/obo/GAZ_00261002 -->

    <owl:NamedIndividual rdf:about="http://purl.obolibrary.org/obo/GAZ_00261002">
        <obo:RO_0001025 rdf:resource="http://purl.obolibrary.org/obo/GAZ_00016178"/>
        <obo:IAO_0000115>A river.</obo:IAO_0000115>
        <oboInOwl:hasOBONamespace>GAZ</oboInOwl:hasOBONamespace>
        <oboInOwl:id>GAZ:00261002</oboInOwl:id>
        <rdfs:label>Zongwe River</rdfs:label>
    </owl:NamedIndividual>
    


    <!-- http://purl.obolibrary.org/obo/GAZ_00261003 -->

    <owl:NamedIndividual rdf:about="http://purl.obolibrary.org/obo/GAZ_00261003">
        <obo:RO_0001025 rdf:resource="http://purl.obolibrary.org/obo/GAZ_00016178"/>
        <obo:IAO_0000115>A river.</obo:IAO_0000115>
        <oboInOwl:hasOBONamespace>GAZ</oboInOwl:hasOBONamespace>
        <oboInOwl:id>GAZ:00261003</oboInOwl:id>
        <rdfs:label>Nangombe River</rdfs:label>
    </owl:NamedIndividual>
    


    <!-- http://purl.obolibrary.org/obo/GAZ_00261004 -->

    <owl:NamedIndividual rdf:about="http://purl.obolibrary.org/obo/GAZ_00261004">
        <obo:RO_0001025 rdf:resource="http://purl.obolibrary.org/obo/GAZ_00016178"/>
        <obo:IAO_0000115>A river.</obo:IAO_0000115>
        <oboInOwl:hasOBONamespace>GAZ</oboInOwl:hasOBONamespace>
        <oboInOwl:id>GAZ:00261004</oboInOwl:id>
        <rdfs:label>Chezya River</rdfs:label>
    </owl:NamedIndividual>
    


    <!-- http://purl.obolibrary.org/obo/GAZ_00261005 -->

    <owl:NamedIndividual rdf:about="http://purl.obolibrary.org/obo/GAZ_00261005">
        <obo:RO_0001025 rdf:resource="http://purl.obolibrary.org/obo/GAZ_00016178"/>
        <obo:IAO_0000115>A river.</obo:IAO_0000115>
        <oboInOwl:hasOBONamespace>GAZ</oboInOwl:hasOBONamespace>
        <oboInOwl:id>GAZ:00261005</oboInOwl:id>
        <rdfs:label>Chibue River</rdfs:label>
    </owl:NamedIndividual>
    


    <!-- http://purl.obolibrary.org/obo/GAZ_00261006 -->

    <owl:NamedIndividual rdf:about="http://purl.obolibrary.org/obo/GAZ_00261006">
        <obo:RO_0001025 rdf:resource="http://purl.obolibrary.org/obo/GAZ_00016178"/>
        <obo:IAO_0000115>A river.</obo:IAO_0000115>
        <oboInOwl:hasOBONamespace>GAZ</oboInOwl:hasOBONamespace>
        <oboInOwl:id>GAZ:00261006</oboInOwl:id>
        <rdfs:label>Lufue River</rdfs:label>
    </owl:NamedIndividual>
    


    <!-- http://purl.obolibrary.org/obo/GAZ_00261009 -->

    <owl:NamedIndividual rdf:about="http://purl.obolibrary.org/obo/GAZ_00261009">
        <obo:IAO_0000115>A dam. Located at Chitungwiza.</obo:IAO_0000115>
        <oboInOwl:hasOBONamespace>GAZ</oboInOwl:hasOBONamespace>
        <oboInOwl:id>GAZ:00261009</oboInOwl:id>
        <rdfs:label>Prince Edward Dam</rdfs:label>
    </owl:NamedIndividual>
    


    <!-- http://purl.obolibrary.org/obo/GAZ_00261010 -->

    <owl:NamedIndividual rdf:about="http://purl.obolibrary.org/obo/GAZ_00261010">
        <obo:IAO_0000115>A man-made lake.</obo:IAO_0000115>
        <oboInOwl:hasOBONamespace>GAZ</oboInOwl:hasOBONamespace>
        <oboInOwl:id>GAZ:00261010</oboInOwl:id>
        <rdfs:label>Lake Robertson</rdfs:label>
    </owl:NamedIndividual>
    


    <!-- http://purl.obolibrary.org/obo/GAZ_00261011 -->

    <owl:NamedIndividual rdf:about="http://purl.obolibrary.org/obo/GAZ_00261011">
        <obo:IAO_0000115>A dam.</obo:IAO_0000115>
        <oboInOwl:hasOBONamespace>GAZ</oboInOwl:hasOBONamespace>
        <oboInOwl:id>GAZ:00261011</oboInOwl:id>
        <rdfs:label>Dutchman&apos;s Pools Dam</rdfs:label>
    </owl:NamedIndividual>
    


    <!-- http://purl.obolibrary.org/obo/GAZ_00261012 -->

    <owl:NamedIndividual rdf:about="http://purl.obolibrary.org/obo/GAZ_00261012">
        <oboInOwl:hasOBONamespace>GAZ</oboInOwl:hasOBONamespace>
        <oboInOwl:id>GAZ:00261012</oboInOwl:id>
        <rdfs:label>Sebakwe Dam</rdfs:label>
    </owl:NamedIndividual>
    


    <!-- http://purl.obolibrary.org/obo/GAZ_22223600 -->

    <owl:NamedIndividual rdf:about="http://purl.obolibrary.org/obo/GAZ_22223600">
        <obo:RO_0001025 rdf:resource="http://purl.obolibrary.org/obo/GAZ_00032660"/>
        <obo:IAO_0000115>A hospital.</obo:IAO_0000115>
        <oboInOwl:hasOBONamespace>GAZ</oboInOwl:hasOBONamespace>
        <oboInOwl:id>GAZ:22223600</oboInOwl:id>
        <rdfs:label>Windhoek Central Hospital</rdfs:label>
    </owl:NamedIndividual>
    


    <!-- http://purl.obolibrary.org/obo/GAZ_22223601 -->

    <owl:NamedIndividual rdf:about="http://purl.obolibrary.org/obo/GAZ_22223601">
        <obo:RO_0001025 rdf:resource="http://purl.obolibrary.org/obo/GAZ_00032654"/>
        <obo:IAO_0000115>A hospital.</obo:IAO_0000115>
        <oboInOwl:hasOBONamespace>GAZ</oboInOwl:hasOBONamespace>
        <oboInOwl:id>GAZ:22223601</oboInOwl:id>
        <rdfs:label>Katutura Hospital</rdfs:label>
    </owl:NamedIndividual>
    


    <!-- http://purl.obolibrary.org/obo/GAZ_22223602 -->

    <owl:NamedIndividual rdf:about="http://purl.obolibrary.org/obo/GAZ_22223602">
        <obo:RO_0001025 rdf:resource="http://purl.obolibrary.org/obo/GAZ_00032654"/>
        <obo:IAO_0000115>A clinic of Katutura State Hospital.</obo:IAO_0000115>
        <oboInOwl:hasOBONamespace>GAZ</oboInOwl:hasOBONamespace>
        <oboInOwl:id>GAZ:22223602</oboInOwl:id>
        <rdfs:label>Katutura Health Centre</rdfs:label>
    </owl:NamedIndividual>
    


    <!-- http://purl.obolibrary.org/obo/GAZ_22223603 -->

    <owl:NamedIndividual rdf:about="http://purl.obolibrary.org/obo/GAZ_22223603">
        <obo:RO_0001025 rdf:resource="http://purl.obolibrary.org/obo/GAZ_00032647"/>
        <obo:IAO_0000115>A clinic of Katutura State Hospital.</obo:IAO_0000115>
        <oboInOwl:hasOBONamespace>GAZ</oboInOwl:hasOBONamespace>
        <oboInOwl:id>GAZ:22223603</oboInOwl:id>
        <rdfs:label>Khomasdal Health Centre</rdfs:label>
    </owl:NamedIndividual>
    


    <!-- http://purl.obolibrary.org/obo/GAZ_22223604 -->

    <owl:NamedIndividual rdf:about="http://purl.obolibrary.org/obo/GAZ_22223604">
        <obo:RO_0001025 rdf:resource="http://purl.obolibrary.org/obo/GAZ_00032646"/>
        <obo:IAO_0000115>A clinic of Katutura State Hospital.</obo:IAO_0000115>
        <oboInOwl:hasOBONamespace>GAZ</oboInOwl:hasOBONamespace>
        <oboInOwl:id>GAZ:22223604</oboInOwl:id>
        <rdfs:label>Baumgartsbrunn Clinic</rdfs:label>
    </owl:NamedIndividual>
    


    <!-- http://purl.obolibrary.org/obo/GAZ_22223605 -->

    <owl:NamedIndividual rdf:about="http://purl.obolibrary.org/obo/GAZ_22223605">
        <obo:RO_0001025 rdf:resource="http://purl.obolibrary.org/obo/GAZ_00032637"/>
        <obo:IAO_0000115>A clinic of Katutura State Hospital.</obo:IAO_0000115>
        <oboInOwl:hasOBONamespace>GAZ</oboInOwl:hasOBONamespace>
        <oboInOwl:id>GAZ:22223605</oboInOwl:id>
        <rdfs:label>Donkerhoek Clinic</rdfs:label>
    </owl:NamedIndividual>
    


    <!-- http://purl.obolibrary.org/obo/GAZ_22223606 -->

    <owl:NamedIndividual rdf:about="http://purl.obolibrary.org/obo/GAZ_22223606">
        <obo:RO_0001025 rdf:resource="http://purl.obolibrary.org/obo/GAZ_00032646"/>
        <obo:IAO_0000115>A clinic of Katutura State Hospital.</obo:IAO_0000115>
        <oboInOwl:hasOBONamespace>GAZ</oboInOwl:hasOBONamespace>
        <oboInOwl:id>GAZ:22223606</oboInOwl:id>
        <rdfs:label>Dordabis Clinic</rdfs:label>
    </owl:NamedIndividual>
    


    <!-- http://purl.obolibrary.org/obo/GAZ_22223607 -->

    <owl:NamedIndividual rdf:about="http://purl.obolibrary.org/obo/GAZ_22223607">
        <obo:RO_0001025 rdf:resource="http://purl.obolibrary.org/obo/GAZ_00239455"/>
        <obo:IAO_0000115>A clinic of Katutura State Hospital.</obo:IAO_0000115>
        <oboInOwl:hasOBONamespace>GAZ</oboInOwl:hasOBONamespace>
        <oboInOwl:id>GAZ:22223607</oboInOwl:id>
        <rdfs:label>Hakahana Clinic</rdfs:label>
    </owl:NamedIndividual>
    


    <!-- http://purl.obolibrary.org/obo/GAZ_22223608 -->

    <owl:NamedIndividual rdf:about="http://purl.obolibrary.org/obo/GAZ_22223608">
        <obo:RO_0001025 rdf:resource="http://purl.obolibrary.org/obo/GAZ_00239455"/>
        <obo:IAO_0000115>A clinic of Katutura State Hospital.</obo:IAO_0000115>
        <oboInOwl:hasOBONamespace>GAZ</oboInOwl:hasOBONamespace>
        <oboInOwl:id>GAZ:22223608</oboInOwl:id>
        <rdfs:label>Okuryangava Clinic</rdfs:label>
    </owl:NamedIndividual>
    


    <!-- http://purl.obolibrary.org/obo/GAZ_22223609 -->

    <owl:NamedIndividual rdf:about="http://purl.obolibrary.org/obo/GAZ_22223609">
        <obo:RO_0001025 rdf:resource="http://purl.obolibrary.org/obo/GAZ_00032656"/>
        <obo:IAO_0000115>A clinic of Katutura State Hospital.</obo:IAO_0000115>
        <oboInOwl:hasOBONamespace>GAZ</oboInOwl:hasOBONamespace>
        <oboInOwl:id>GAZ:22223609</oboInOwl:id>
        <rdfs:label>Robert Mugabe Clinic</rdfs:label>
    </owl:NamedIndividual>
    


    <!-- http://purl.obolibrary.org/obo/GAZ_22223610 -->

    <owl:NamedIndividual rdf:about="http://purl.obolibrary.org/obo/GAZ_22223610">
        <obo:RO_0001025 rdf:resource="http://purl.obolibrary.org/obo/GAZ_00032650"/>
        <obo:IAO_0000115>A clinic of Katutura State Hospital.</obo:IAO_0000115>
        <oboInOwl:hasOBONamespace>GAZ</oboInOwl:hasOBONamespace>
        <oboInOwl:id>GAZ:22223610</oboInOwl:id>
        <rdfs:label>Wanaheda Clinic</rdfs:label>
    </owl:NamedIndividual>
    


    <!-- 
    ///////////////////////////////////////////////////////////////////////////////////////
    //
    // Annotations
    //
    ///////////////////////////////////////////////////////////////////////////////////////
     -->

    <rdf:Description rdf:about="http://purl.obolibrary.org/obo/GAZ_00009435">
        <rdfs:label>Region (Namibia)</rdfs:label>
        <oboInOwl:id>GAZ:00009435</oboInOwl:id>
        <oboInOwl:hasOBONamespace>GAZ</oboInOwl:hasOBONamespace>
    </rdf:Description>
    <rdf:Description rdf:about="http://purl.obolibrary.org/obo/GAZ_00014897">
        <rdfs:label>Kunene Region</rdfs:label>
        <oboInOwl:id>GAZ:00014897</oboInOwl:id>
        <oboInOwl:hasOBONamespace>GAZ</oboInOwl:hasOBONamespace>
        <obo:IAO_0000115>One of the thirteen regions of Namibia. The largest town and capital is Opuwo.</obo:IAO_0000115>
    </rdf:Description>
    <rdf:Description rdf:about="http://purl.obolibrary.org/obo/GAZ_00014898">
        <rdfs:label>Khomas Region</rdfs:label>
        <obo:IAO_0000115>One of the thirteen regions of Namibia. Khomas contains the capital city of Namibia, Windhoek.</obo:IAO_0000115>
        <oboInOwl:hasOBONamespace>GAZ</oboInOwl:hasOBONamespace>
        <oboInOwl:id>GAZ:00014898</oboInOwl:id>
    </rdf:Description>
    <rdf:Description rdf:about="http://purl.obolibrary.org/obo/GAZ_00014899">
        <rdfs:label>Omaheke Region</rdfs:label>
        <obo:IAO_0000115>One of the thirteen regions of Namibia. Omaheke lies on the eastern border of Namibia.</obo:IAO_0000115>
        <oboInOwl:id>GAZ:00014899</oboInOwl:id>
        <oboInOwl:hasOBONamespace>GAZ</oboInOwl:hasOBONamespace>
    </rdf:Description>
    <rdf:Description rdf:about="http://purl.obolibrary.org/obo/GAZ_00014900">
        <oboInOwl:id>GAZ:00014900</oboInOwl:id>
        <oboInOwl:hasOBONamespace>GAZ</oboInOwl:hasOBONamespace>
        <obo:IAO_0000115>The southernmost region of Namibia.</obo:IAO_0000115>
        <rdfs:label>Karas Region</rdfs:label>
    </rdf:Description>
    <rdf:Description rdf:about="http://purl.obolibrary.org/obo/GAZ_00014901">
        <obo:IAO_0000115>One of the thirteen regions of Namibia.</obo:IAO_0000115>
        <rdfs:label>Oshikoto Region</rdfs:label>
        <oboInOwl:id>GAZ:00014901</oboInOwl:id>
        <oboInOwl:hasOBONamespace>GAZ</oboInOwl:hasOBONamespace>
    </rdf:Description>
    <rdf:Description rdf:about="http://purl.obolibrary.org/obo/GAZ_00014902">
        <rdfs:label>Okavango Region</rdfs:label>
        <obo:IAO_0000115>One of the thirteen regions of Namibia.</obo:IAO_0000115>
        <oboInOwl:id>GAZ:00014902</oboInOwl:id>
        <oboInOwl:hasOBONamespace>GAZ</oboInOwl:hasOBONamespace>
    </rdf:Description>
    <rdf:Description rdf:about="http://purl.obolibrary.org/obo/GAZ_00014903">
        <obo:IAO_0000115>One of the thirteen regions of Namibia.</obo:IAO_0000115>
        <rdfs:label>Oshana Region</rdfs:label>
        <oboInOwl:id>GAZ:00014903</oboInOwl:id>
        <oboInOwl:hasOBONamespace>GAZ</oboInOwl:hasOBONamespace>
    </rdf:Description>
    <rdf:Description rdf:about="http://purl.obolibrary.org/obo/GAZ_00014904">
        <obo:IAO_0000115>One of the thirteen regions of Namibia.</obo:IAO_0000115>
        <rdfs:label>Omusati Region</rdfs:label>
        <oboInOwl:id>GAZ:00014904</oboInOwl:id>
        <oboInOwl:hasOBONamespace>GAZ</oboInOwl:hasOBONamespace>
    </rdf:Description>
    <rdf:Description rdf:about="http://purl.obolibrary.org/obo/GAZ_00014905">
        <oboInOwl:id>GAZ:00014905</oboInOwl:id>
        <obo:IAO_0000115>One of the thirteen regions of Namibia.</obo:IAO_0000115>
        <oboInOwl:hasOBONamespace>GAZ</oboInOwl:hasOBONamespace>
        <rdfs:label>Ohangwena Region</rdfs:label>
    </rdf:Description>
    <rdf:Description rdf:about="http://purl.obolibrary.org/obo/GAZ_00014906">
        <oboInOwl:id>GAZ:00014906</oboInOwl:id>
        <obo:IAO_0000115>One of the 13 regions of Namibia. It comprises the Swakopmund magisterial district up to the Ugab River and includes Walvis Bay, Omaruru and Karibib magisterial districts.</obo:IAO_0000115>
        <rdfs:label>Erongo Region</rdfs:label>
        <oboInOwl:hasOBONamespace>GAZ</oboInOwl:hasOBONamespace>
    </rdf:Description>
    <rdf:Description rdf:about="http://purl.obolibrary.org/obo/GAZ_00014907">
        <oboInOwl:id>GAZ:00014907</oboInOwl:id>
        <obo:IAO_0000115>One of the thirteen regions of Namibia.</obo:IAO_0000115>
        <oboInOwl:hasOBONamespace>GAZ</oboInOwl:hasOBONamespace>
        <rdfs:label>Otjozondjupa Region</rdfs:label>
    </rdf:Description>
    <rdf:Description rdf:about="http://purl.obolibrary.org/obo/GAZ_00014908">
        <obo:IAO_0000115>One of the thirteen regions of Namibia.</obo:IAO_0000115>
        <rdfs:label>Hardap Region</rdfs:label>
        <oboInOwl:id>GAZ:00014908</oboInOwl:id>
        <oboInOwl:hasOBONamespace>GAZ</oboInOwl:hasOBONamespace>
    </rdf:Description>
</rdf:RDF>



<!-- Generated by the OWL API (version 4.5.6) https://github.com/owlcs/owlapi -->

