<?xml version="1.0"?>
<rdf:RDF xmlns="http://purl.obolibrary.org/obo/gaz/subsets/countries/New_Zealand.owl#"
     xml:base="http://purl.obolibrary.org/obo/gaz/subsets/countries/New_Zealand.owl"
     xmlns:dc="http://purl.org/dc/elements/1.1/"
     xmlns:obo="http://purl.obolibrary.org/obo/"
     xmlns:owl="http://www.w3.org/2002/07/owl#"
     xmlns:rdf="http://www.w3.org/1999/02/22-rdf-syntax-ns#"
     xmlns:xml="http://www.w3.org/XML/1998/namespace"
     xmlns:xsd="http://www.w3.org/2001/XMLSchema#"
     xmlns:envo="http://purl.obolibrary.org/obo/envo#"
     xmlns:rdfs="http://www.w3.org/2000/01/rdf-schema#"
     xmlns:oboInOwl="http://www.geneontology.org/formats/oboInOwl#">
    <owl:Ontology rdf:about="http://purl.obolibrary.org/obo/gaz/subsets/countries/New_Zealand.owl">
        <owl:imports rdf:resource="http://purl.obolibrary.org/obo/gaz/imports/envo_import.owl"/>
        <owl:imports rdf:resource="http://purl.obolibrary.org/obo/gaz/imports/ro_import.owl"/>
    </owl:Ontology>
    


    <!-- 
    ///////////////////////////////////////////////////////////////////////////////////////
    //
    // Annotation properties
    //
    ///////////////////////////////////////////////////////////////////////////////////////
     -->

    


    <!-- http://purl.obolibrary.org/obo/IAO_0000115 -->

    <owl:AnnotationProperty rdf:about="http://purl.obolibrary.org/obo/IAO_0000115"/>
    


    <!-- http://www.geneontology.org/formats/oboInOwl#hasOBONamespace -->

    <owl:AnnotationProperty rdf:about="http://www.geneontology.org/formats/oboInOwl#hasOBONamespace"/>
    


    <!-- http://www.geneontology.org/formats/oboInOwl#id -->

    <owl:AnnotationProperty rdf:about="http://www.geneontology.org/formats/oboInOwl#id"/>
    


    <!-- 
    ///////////////////////////////////////////////////////////////////////////////////////
    //
    // Object Properties
    //
    ///////////////////////////////////////////////////////////////////////////////////////
     -->

    


    <!-- http://purl.obolibrary.org/obo/RO_0001025 -->

    <owl:ObjectProperty rdf:about="http://purl.obolibrary.org/obo/RO_0001025"/>
    


    <!-- 
    ///////////////////////////////////////////////////////////////////////////////////////
    //
    // Classes
    //
    ///////////////////////////////////////////////////////////////////////////////////////
     -->

    


    <!-- http://purl.obolibrary.org/obo/ENVO_00000004 -->

    <owl:Class rdf:about="http://purl.obolibrary.org/obo/ENVO_00000004"/>
    


    <!-- http://purl.obolibrary.org/obo/ENVO_00000020 -->

    <owl:Class rdf:about="http://purl.obolibrary.org/obo/ENVO_00000020"/>
    


    <!-- http://purl.obolibrary.org/obo/ENVO_00000032 -->

    <owl:Class rdf:about="http://purl.obolibrary.org/obo/ENVO_00000032"/>
    


    <!-- http://purl.obolibrary.org/obo/ENVO_00000062 -->

    <owl:Class rdf:about="http://purl.obolibrary.org/obo/ENVO_00000062"/>
    


    <!-- http://purl.obolibrary.org/obo/ENVO_00000087 -->

    <owl:Class rdf:about="http://purl.obolibrary.org/obo/ENVO_00000087"/>
    


    <!-- http://purl.obolibrary.org/obo/ENVO_00000100 -->

    <owl:Class rdf:about="http://purl.obolibrary.org/obo/ENVO_00000100"/>
    


    <!-- http://purl.obolibrary.org/obo/ENVO_00000106 -->

    <owl:Class rdf:about="http://purl.obolibrary.org/obo/ENVO_00000106"/>
    


    <!-- http://purl.obolibrary.org/obo/ENVO_00000167 -->

    <owl:Class rdf:about="http://purl.obolibrary.org/obo/ENVO_00000167"/>
    


    <!-- http://purl.obolibrary.org/obo/ENVO_00000220 -->

    <owl:Class rdf:about="http://purl.obolibrary.org/obo/ENVO_00000220"/>
    


    <!-- http://purl.obolibrary.org/obo/ENVO_00000222 -->

    <owl:Class rdf:about="http://purl.obolibrary.org/obo/ENVO_00000222"/>
    


    <!-- http://purl.obolibrary.org/obo/ENVO_00000305 -->

    <owl:Class rdf:about="http://purl.obolibrary.org/obo/ENVO_00000305"/>
    


    <!-- http://purl.obolibrary.org/obo/ENVO_00000354 -->

    <owl:Class rdf:about="http://purl.obolibrary.org/obo/ENVO_00000354"/>
    


    <!-- http://purl.obolibrary.org/obo/ENVO_00000475 -->

    <owl:Class rdf:about="http://purl.obolibrary.org/obo/ENVO_00000475"/>
    


    <!-- http://purl.obolibrary.org/obo/ENVO_00000856 -->

    <owl:Class rdf:about="http://purl.obolibrary.org/obo/ENVO_00000856"/>
    


    <!-- http://purl.obolibrary.org/obo/GAZ_00004759 -->

    <owl:Class rdf:about="http://purl.obolibrary.org/obo/GAZ_00004759"/>
    


    <!-- http://purl.obolibrary.org/obo/GAZ_00004760 -->

    <owl:Class rdf:about="http://purl.obolibrary.org/obo/GAZ_00004760">
        <rdfs:subClassOf rdf:resource="http://purl.obolibrary.org/obo/GAZ_00004759"/>
    </owl:Class>
    


    <!-- http://purl.obolibrary.org/obo/GAZ_00004762 -->

    <owl:Class rdf:about="http://purl.obolibrary.org/obo/GAZ_00004762"/>
    


    <!-- http://purl.obolibrary.org/obo/GAZ_00004767 -->

    <owl:Class rdf:about="http://purl.obolibrary.org/obo/GAZ_00004767">
        <rdfs:subClassOf rdf:resource="http://purl.obolibrary.org/obo/GAZ_00004759"/>
    </owl:Class>
    


    <!-- http://purl.obolibrary.org/obo/GAZ_00004768 -->

    <owl:Class rdf:about="http://purl.obolibrary.org/obo/GAZ_00004768">
        <rdfs:subClassOf rdf:resource="http://purl.obolibrary.org/obo/GAZ_00004762"/>
    </owl:Class>
    


    <!-- http://purl.obolibrary.org/obo/GAZ_00004770 -->

    <owl:Class rdf:about="http://purl.obolibrary.org/obo/GAZ_00004770">
        <rdfs:subClassOf rdf:resource="http://purl.obolibrary.org/obo/GAZ_00004762"/>
    </owl:Class>
    


    <!-- http://purl.obolibrary.org/obo/GAZ_00004772 -->

    <owl:Class rdf:about="http://purl.obolibrary.org/obo/GAZ_00004772">
        <rdfs:subClassOf rdf:resource="http://purl.obolibrary.org/obo/GAZ_00004759"/>
    </owl:Class>
    


    <!-- http://purl.obolibrary.org/obo/GAZ_00004773 -->

    <owl:Class rdf:about="http://purl.obolibrary.org/obo/GAZ_00004773">
        <rdfs:subClassOf rdf:resource="http://purl.obolibrary.org/obo/GAZ_00004762"/>
    </owl:Class>
    


    <!-- http://purl.obolibrary.org/obo/GAZ_00004777 -->

    <owl:Class rdf:about="http://purl.obolibrary.org/obo/GAZ_00004777">
        <rdfs:subClassOf rdf:resource="http://purl.obolibrary.org/obo/GAZ_00004759"/>
    </owl:Class>
    


    <!-- http://purl.obolibrary.org/obo/GAZ_00004781 -->

    <owl:Class rdf:about="http://purl.obolibrary.org/obo/GAZ_00004781">
        <rdfs:subClassOf rdf:resource="http://purl.obolibrary.org/obo/GAZ_00004759"/>
    </owl:Class>
    


    <!-- http://purl.obolibrary.org/obo/GAZ_00007723 -->

    <owl:Class rdf:about="http://purl.obolibrary.org/obo/GAZ_00007723">
        <rdfs:subClassOf rdf:resource="http://purl.obolibrary.org/obo/GAZ_00004759"/>
    </owl:Class>
    


    <!-- http://purl.obolibrary.org/obo/GAZ_00007724 -->

    <owl:Class rdf:about="http://purl.obolibrary.org/obo/GAZ_00007724">
        <rdfs:subClassOf rdf:resource="http://purl.obolibrary.org/obo/GAZ_00004762"/>
    </owl:Class>
    


    <!-- http://purl.obolibrary.org/obo/GAZ_00008561 -->

    <owl:Class rdf:about="http://purl.obolibrary.org/obo/GAZ_00008561">
        <rdfs:subClassOf rdf:resource="http://purl.obolibrary.org/obo/GAZ_00004762"/>
    </owl:Class>
    


    <!-- http://purl.obolibrary.org/obo/GAZ_00008562 -->

    <owl:Class rdf:about="http://purl.obolibrary.org/obo/GAZ_00008562">
        <rdfs:subClassOf rdf:resource="http://purl.obolibrary.org/obo/GAZ_00004759"/>
    </owl:Class>
    


    <!-- http://purl.obolibrary.org/obo/GAZ_00008564 -->

    <owl:Class rdf:about="http://purl.obolibrary.org/obo/GAZ_00008564">
        <rdfs:subClassOf rdf:resource="http://purl.obolibrary.org/obo/GAZ_00004759"/>
    </owl:Class>
    


    <!-- http://purl.obolibrary.org/obo/GAZ_00008565 -->

    <owl:Class rdf:about="http://purl.obolibrary.org/obo/GAZ_00008565">
        <rdfs:subClassOf rdf:resource="http://purl.obolibrary.org/obo/GAZ_00004759"/>
    </owl:Class>
    


    <!-- http://purl.obolibrary.org/obo/GAZ_00008568 -->

    <owl:Class rdf:about="http://purl.obolibrary.org/obo/GAZ_00008568">
        <rdfs:subClassOf rdf:resource="http://purl.obolibrary.org/obo/GAZ_00004759"/>
    </owl:Class>
    


    <!-- http://purl.obolibrary.org/obo/GAZ_00008569 -->

    <owl:Class rdf:about="http://purl.obolibrary.org/obo/GAZ_00008569">
        <rdfs:subClassOf rdf:resource="http://purl.obolibrary.org/obo/GAZ_00004759"/>
    </owl:Class>
    


    <!-- http://purl.obolibrary.org/obo/GAZ_00008570 -->

    <owl:Class rdf:about="http://purl.obolibrary.org/obo/GAZ_00008570">
        <rdfs:subClassOf rdf:resource="http://purl.obolibrary.org/obo/GAZ_00004762"/>
    </owl:Class>
    


    <!-- http://purl.obolibrary.org/obo/GAZ_00008571 -->

    <owl:Class rdf:about="http://purl.obolibrary.org/obo/GAZ_00008571">
        <rdfs:subClassOf rdf:resource="http://purl.obolibrary.org/obo/GAZ_00004762"/>
    </owl:Class>
    


    <!-- http://purl.obolibrary.org/obo/GAZ_00008572 -->

    <owl:Class rdf:about="http://purl.obolibrary.org/obo/GAZ_00008572">
        <rdfs:subClassOf rdf:resource="http://purl.obolibrary.org/obo/GAZ_00004759"/>
    </owl:Class>
    


    <!-- http://purl.obolibrary.org/obo/GAZ_00009534 -->

    <owl:Class rdf:about="http://purl.obolibrary.org/obo/GAZ_00009534">
        <rdfs:subClassOf rdf:resource="http://purl.obolibrary.org/obo/GAZ_00004762"/>
    </owl:Class>
    


    <!-- http://purl.obolibrary.org/obo/GAZ_00009760 -->

    <owl:Class rdf:about="http://purl.obolibrary.org/obo/GAZ_00009760">
        <rdfs:subClassOf rdf:resource="http://purl.obolibrary.org/obo/GAZ_00004762"/>
    </owl:Class>
    


    <!-- http://purl.obolibrary.org/obo/GAZ_00009762 -->

    <owl:Class rdf:about="http://purl.obolibrary.org/obo/GAZ_00009762">
        <rdfs:subClassOf rdf:resource="http://purl.obolibrary.org/obo/GAZ_00004762"/>
    </owl:Class>
    


    <!-- http://purl.obolibrary.org/obo/GAZ_00009763 -->

    <owl:Class rdf:about="http://purl.obolibrary.org/obo/GAZ_00009763">
        <rdfs:subClassOf rdf:resource="http://purl.obolibrary.org/obo/GAZ_00004762"/>
    </owl:Class>
    


    <!-- http://purl.obolibrary.org/obo/GAZ_00009776 -->

    <owl:Class rdf:about="http://purl.obolibrary.org/obo/GAZ_00009776">
        <rdfs:subClassOf rdf:resource="http://purl.obolibrary.org/obo/GAZ_00004762"/>
    </owl:Class>
    


    <!-- http://purl.obolibrary.org/obo/GAZ_00010240 -->

    <owl:Class rdf:about="http://purl.obolibrary.org/obo/GAZ_00010240">
        <rdfs:subClassOf rdf:resource="http://purl.obolibrary.org/obo/GAZ_00004762"/>
    </owl:Class>
    


    <!-- http://purl.obolibrary.org/obo/GAZ_00010241 -->

    <owl:Class rdf:about="http://purl.obolibrary.org/obo/GAZ_00010241">
        <rdfs:subClassOf rdf:resource="http://purl.obolibrary.org/obo/GAZ_00004762"/>
    </owl:Class>
    


    <!-- http://purl.obolibrary.org/obo/GAZ_00010245 -->

    <owl:Class rdf:about="http://purl.obolibrary.org/obo/GAZ_00010245">
        <rdfs:subClassOf rdf:resource="http://purl.obolibrary.org/obo/GAZ_00004762"/>
    </owl:Class>
    


    <!-- http://purl.obolibrary.org/obo/GAZ_00010246 -->

    <owl:Class rdf:about="http://purl.obolibrary.org/obo/GAZ_00010246">
        <rdfs:subClassOf rdf:resource="http://purl.obolibrary.org/obo/GAZ_00004762"/>
    </owl:Class>
    


    <!-- http://purl.obolibrary.org/obo/GAZ_00010247 -->

    <owl:Class rdf:about="http://purl.obolibrary.org/obo/GAZ_00010247">
        <rdfs:subClassOf rdf:resource="http://purl.obolibrary.org/obo/GAZ_00004762"/>
    </owl:Class>
    


    <!-- http://purl.obolibrary.org/obo/GAZ_00010250 -->

    <owl:Class rdf:about="http://purl.obolibrary.org/obo/GAZ_00010250">
        <rdfs:subClassOf rdf:resource="http://purl.obolibrary.org/obo/GAZ_00004762"/>
    </owl:Class>
    


    <!-- http://purl.obolibrary.org/obo/GAZ_00010251 -->

    <owl:Class rdf:about="http://purl.obolibrary.org/obo/GAZ_00010251">
        <rdfs:subClassOf rdf:resource="http://purl.obolibrary.org/obo/GAZ_00004762"/>
    </owl:Class>
    


    <!-- http://purl.obolibrary.org/obo/GAZ_00010254 -->

    <owl:Class rdf:about="http://purl.obolibrary.org/obo/GAZ_00010254">
        <rdfs:subClassOf rdf:resource="http://purl.obolibrary.org/obo/GAZ_00004762"/>
    </owl:Class>
    


    <!-- http://purl.obolibrary.org/obo/GAZ_00010256 -->

    <owl:Class rdf:about="http://purl.obolibrary.org/obo/GAZ_00010256">
        <rdfs:subClassOf rdf:resource="http://purl.obolibrary.org/obo/GAZ_00004759"/>
    </owl:Class>
    


    <!-- http://purl.obolibrary.org/obo/GAZ_00010257 -->

    <owl:Class rdf:about="http://purl.obolibrary.org/obo/GAZ_00010257">
        <rdfs:subClassOf rdf:resource="http://purl.obolibrary.org/obo/GAZ_00004762"/>
    </owl:Class>
    


    <!-- http://purl.obolibrary.org/obo/GAZ_00146180 -->

    <owl:Class rdf:about="http://purl.obolibrary.org/obo/GAZ_00146180">
        <rdfs:subClassOf rdf:resource="http://purl.obolibrary.org/obo/GAZ_00004762"/>
    </owl:Class>
    


    <!-- http://purl.obolibrary.org/obo/GAZ_00146181 -->

    <owl:Class rdf:about="http://purl.obolibrary.org/obo/GAZ_00146181">
        <rdfs:subClassOf rdf:resource="http://purl.obolibrary.org/obo/GAZ_00004762"/>
    </owl:Class>
    


    <!-- http://purl.obolibrary.org/obo/GAZ_22224487 -->

    <owl:Class rdf:about="http://purl.obolibrary.org/obo/GAZ_22224487">
        <rdfs:subClassOf rdf:resource="http://purl.obolibrary.org/obo/GAZ_00004762"/>
    </owl:Class>
    


    <!-- 
    ///////////////////////////////////////////////////////////////////////////////////////
    //
    // Individuals
    //
    ///////////////////////////////////////////////////////////////////////////////////////
     -->

    


    <!-- http://purl.obolibrary.org/obo/GAZ_00000469 -->

    <owl:NamedIndividual rdf:about="http://purl.obolibrary.org/obo/GAZ_00000469">
        <obo:IAO_0000115>A nation in the south-western Pacific Ocean comprising two large islands (the North Island and the South Island) and numerous smaller islands, most notably Stewart Island/Rakiura and the Chatham Islands.</obo:IAO_0000115>
        <oboInOwl:hasOBONamespace>GAZ</oboInOwl:hasOBONamespace>
        <oboInOwl:id>GAZ:00000469</oboInOwl:id>
        <rdfs:label>New Zealand</rdfs:label>
    </owl:NamedIndividual>
    


    <!-- http://purl.obolibrary.org/obo/GAZ_00004759 -->

    <owl:NamedIndividual rdf:about="http://purl.obolibrary.org/obo/GAZ_00004759">
        <obo:RO_0001025 rdf:resource="http://purl.obolibrary.org/obo/GAZ_00000469"/>
    </owl:NamedIndividual>
    


    <!-- http://purl.obolibrary.org/obo/GAZ_00004760 -->

    <owl:NamedIndividual rdf:about="http://purl.obolibrary.org/obo/GAZ_00004760">
        <obo:RO_0001025 rdf:resource="http://purl.obolibrary.org/obo/GAZ_00004765"/>
    </owl:NamedIndividual>
    


    <!-- http://purl.obolibrary.org/obo/GAZ_00004762 -->

    <owl:NamedIndividual rdf:about="http://purl.obolibrary.org/obo/GAZ_00004762">
        <obo:RO_0001025 rdf:resource="http://purl.obolibrary.org/obo/GAZ_00000469"/>
    </owl:NamedIndividual>
    


    <!-- http://purl.obolibrary.org/obo/GAZ_00004764 -->

    <owl:NamedIndividual rdf:about="http://purl.obolibrary.org/obo/GAZ_00004764">
        <obo:RO_0001025 rdf:resource="http://purl.obolibrary.org/obo/GAZ_00000469"/>
        <obo:IAO_0000115>The larger of the two major islands of New Zealand, the other being the more populous North Island.</obo:IAO_0000115>
        <oboInOwl:hasOBONamespace>GAZ</oboInOwl:hasOBONamespace>
        <oboInOwl:id>GAZ:00004764</oboInOwl:id>
        <rdfs:label>South Island</rdfs:label>
    </owl:NamedIndividual>
    


    <!-- http://purl.obolibrary.org/obo/GAZ_00004765 -->

    <owl:NamedIndividual rdf:about="http://purl.obolibrary.org/obo/GAZ_00004765">
        <obo:RO_0001025 rdf:resource="http://purl.obolibrary.org/obo/GAZ_00000469"/>
        <obo:IAO_0000115>One of the two main islands of New Zealand, the other being the South Island.</obo:IAO_0000115>
        <oboInOwl:hasOBONamespace>GAZ</oboInOwl:hasOBONamespace>
        <oboInOwl:id>GAZ:00004765</oboInOwl:id>
        <rdfs:label>North Island</rdfs:label>
    </owl:NamedIndividual>
    


    <!-- http://purl.obolibrary.org/obo/GAZ_00004766 -->

    <owl:NamedIndividual rdf:about="http://purl.obolibrary.org/obo/GAZ_00004766">
        <obo:RO_0001025 rdf:resource="http://purl.obolibrary.org/obo/GAZ_00009534"/>
        <oboInOwl:hasOBONamespace>GAZ</oboInOwl:hasOBONamespace>
        <oboInOwl:id>GAZ:00004766</oboInOwl:id>
        <rdfs:label>Western Springs Lake</rdfs:label>
    </owl:NamedIndividual>
    


    <!-- http://purl.obolibrary.org/obo/GAZ_00004767 -->

    <owl:NamedIndividual rdf:about="http://purl.obolibrary.org/obo/GAZ_00004767">
        <obo:RO_0001025 rdf:resource="http://purl.obolibrary.org/obo/GAZ_00004764"/>
    </owl:NamedIndividual>
    


    <!-- http://purl.obolibrary.org/obo/GAZ_00004768 -->

    <owl:NamedIndividual rdf:about="http://purl.obolibrary.org/obo/GAZ_00004768">
        <obo:RO_0001025 rdf:resource="http://purl.obolibrary.org/obo/GAZ_00004767"/>
    </owl:NamedIndividual>
    


    <!-- http://purl.obolibrary.org/obo/GAZ_00004769 -->

    <owl:NamedIndividual rdf:about="http://purl.obolibrary.org/obo/GAZ_00004769">
        <obo:RO_0001025 rdf:resource="http://purl.obolibrary.org/obo/GAZ_00000469"/>
        <oboInOwl:hasOBONamespace>GAZ</oboInOwl:hasOBONamespace>
        <oboInOwl:id>GAZ:00004769</oboInOwl:id>
        <rdfs:label>Henkes Bay</rdfs:label>
    </owl:NamedIndividual>
    


    <!-- http://purl.obolibrary.org/obo/GAZ_00004770 -->

    <owl:NamedIndividual rdf:about="http://purl.obolibrary.org/obo/GAZ_00004770">
        <obo:RO_0001025 rdf:resource="http://purl.obolibrary.org/obo/GAZ_00012589"/>
    </owl:NamedIndividual>
    


    <!-- http://purl.obolibrary.org/obo/GAZ_00004771 -->

    <owl:NamedIndividual rdf:about="http://purl.obolibrary.org/obo/GAZ_00004771">
        <obo:RO_0001025 rdf:resource="http://purl.obolibrary.org/obo/GAZ_00004770"/>
        <oboInOwl:hasOBONamespace>GAZ</oboInOwl:hasOBONamespace>
        <oboInOwl:id>GAZ:00004771</oboInOwl:id>
        <rdfs:label>Seed Control Station</rdfs:label>
    </owl:NamedIndividual>
    


    <!-- http://purl.obolibrary.org/obo/GAZ_00004772 -->

    <owl:NamedIndividual rdf:about="http://purl.obolibrary.org/obo/GAZ_00004772">
        <obo:RO_0001025 rdf:resource="http://purl.obolibrary.org/obo/GAZ_00004765"/>
        <obo:RO_0001025 rdf:resource="http://purl.obolibrary.org/obo/GAZ_00010255"/>
    </owl:NamedIndividual>
    


    <!-- http://purl.obolibrary.org/obo/GAZ_00004773 -->

    <owl:NamedIndividual rdf:about="http://purl.obolibrary.org/obo/GAZ_00004773">
        <obo:RO_0001025 rdf:resource="http://purl.obolibrary.org/obo/GAZ_00004772"/>
    </owl:NamedIndividual>
    


    <!-- http://purl.obolibrary.org/obo/GAZ_00004774 -->

    <owl:NamedIndividual rdf:about="http://purl.obolibrary.org/obo/GAZ_00004774">
        <obo:RO_0001025 rdf:resource="http://purl.obolibrary.org/obo/GAZ_00008572"/>
        <obo:IAO_0000115>The third-largest island of New Zealand. It lies 30 km south of the South Island, across Foveaux Strait.</obo:IAO_0000115>
        <oboInOwl:hasOBONamespace>GAZ</oboInOwl:hasOBONamespace>
        <oboInOwl:id>GAZ:00004774</oboInOwl:id>
        <rdfs:label>Stewart Island</rdfs:label>
    </owl:NamedIndividual>
    


    <!-- http://purl.obolibrary.org/obo/GAZ_00004777 -->

    <owl:NamedIndividual rdf:about="http://purl.obolibrary.org/obo/GAZ_00004777">
        <obo:RO_0001025 rdf:resource="http://purl.obolibrary.org/obo/GAZ_00004764"/>
    </owl:NamedIndividual>
    


    <!-- http://purl.obolibrary.org/obo/GAZ_00004778 -->

    <owl:NamedIndividual rdf:about="http://purl.obolibrary.org/obo/GAZ_00004778">
        <obo:RO_0001025 rdf:resource="http://purl.obolibrary.org/obo/GAZ_00004777"/>
        <oboInOwl:hasOBONamespace>GAZ</oboInOwl:hasOBONamespace>
        <oboInOwl:id>GAZ:00004778</oboInOwl:id>
        <rdfs:label>Westland District</rdfs:label>
    </owl:NamedIndividual>
    


    <!-- http://purl.obolibrary.org/obo/GAZ_00004779 -->

    <owl:NamedIndividual rdf:about="http://purl.obolibrary.org/obo/GAZ_00004779">
        <obo:RO_0001025 rdf:resource="http://purl.obolibrary.org/obo/GAZ_00004778"/>
        <oboInOwl:hasOBONamespace>GAZ</oboInOwl:hasOBONamespace>
        <oboInOwl:id>GAZ:00004779</oboInOwl:id>
        <rdfs:label>Okarito State Forest</rdfs:label>
    </owl:NamedIndividual>
    


    <!-- http://purl.obolibrary.org/obo/GAZ_00004780 -->

    <owl:NamedIndividual rdf:about="http://purl.obolibrary.org/obo/GAZ_00004780">
        <obo:RO_0001025 rdf:resource="http://purl.obolibrary.org/obo/GAZ_00004779"/>
        <oboInOwl:hasOBONamespace>GAZ</oboInOwl:hasOBONamespace>
        <oboInOwl:id>GAZ:00004780</oboInOwl:id>
        <rdfs:label>Okarito Road</rdfs:label>
    </owl:NamedIndividual>
    


    <!-- http://purl.obolibrary.org/obo/GAZ_00004781 -->

    <owl:NamedIndividual rdf:about="http://purl.obolibrary.org/obo/GAZ_00004781">
        <obo:RO_0001025 rdf:resource="http://purl.obolibrary.org/obo/GAZ_00004765"/>
    </owl:NamedIndividual>
    


    <!-- http://purl.obolibrary.org/obo/GAZ_00004782 -->

    <owl:NamedIndividual rdf:about="http://purl.obolibrary.org/obo/GAZ_00004782">
        <obo:RO_0001025 rdf:resource="http://purl.obolibrary.org/obo/GAZ_00009541"/>
        <oboInOwl:hasOBONamespace>GAZ</oboInOwl:hasOBONamespace>
        <oboInOwl:id>GAZ:00004782</oboInOwl:id>
        <rdfs:label>Taupo</rdfs:label>
    </owl:NamedIndividual>
    


    <!-- http://purl.obolibrary.org/obo/GAZ_00004783 -->

    <owl:NamedIndividual rdf:about="http://purl.obolibrary.org/obo/GAZ_00004783">
        <obo:RO_0001025 rdf:resource="http://purl.obolibrary.org/obo/GAZ_00004782"/>
        <oboInOwl:hasOBONamespace>GAZ</oboInOwl:hasOBONamespace>
        <oboInOwl:id>GAZ:00004783</oboInOwl:id>
        <rdfs:label>Kaimanawa State Forest Park</rdfs:label>
    </owl:NamedIndividual>
    


    <!-- http://purl.obolibrary.org/obo/GAZ_00006914 -->

    <owl:NamedIndividual rdf:about="http://purl.obolibrary.org/obo/GAZ_00006914">
        <obo:RO_0001025 rdf:resource="http://purl.obolibrary.org/obo/GAZ_00009560"/>
        <obo:IAO_0000115>An island on the Nukunonu Atoll.</obo:IAO_0000115>
        <oboInOwl:hasOBONamespace>GAZ</oboInOwl:hasOBONamespace>
        <oboInOwl:id>GAZ:00006914</oboInOwl:id>
        <rdfs:label>Tokelau</rdfs:label>
    </owl:NamedIndividual>
    


    <!-- http://purl.obolibrary.org/obo/GAZ_00006949 -->

    <owl:NamedIndividual rdf:about="http://purl.obolibrary.org/obo/GAZ_00006949">
        <obo:RO_0001025 rdf:resource="http://purl.obolibrary.org/obo/GAZ_00000469"/>
        <obo:IAO_0000115>A group of atolls in the South Pacific Ocean.</obo:IAO_0000115>
        <oboInOwl:hasOBONamespace>GAZ</oboInOwl:hasOBONamespace>
        <oboInOwl:id>GAZ:00006949</oboInOwl:id>
        <rdfs:label>Tokelau Islands</rdfs:label>
    </owl:NamedIndividual>
    


    <!-- http://purl.obolibrary.org/obo/GAZ_00006950 -->

    <owl:NamedIndividual rdf:about="http://purl.obolibrary.org/obo/GAZ_00006950">
        <obo:RO_0001025 rdf:resource="http://purl.obolibrary.org/obo/GAZ_00006949"/>
        <obo:IAO_0000115>An atoll within Tokelau in the south Pacific Ocean.</obo:IAO_0000115>
        <oboInOwl:hasOBONamespace>GAZ</oboInOwl:hasOBONamespace>
        <oboInOwl:id>GAZ:00006950</oboInOwl:id>
        <rdfs:label>Nukunonu Atoll</rdfs:label>
    </owl:NamedIndividual>
    


    <!-- http://purl.obolibrary.org/obo/GAZ_00006951 -->

    <owl:NamedIndividual rdf:about="http://purl.obolibrary.org/obo/GAZ_00006951">
        <obo:RO_0001025 rdf:resource="http://purl.obolibrary.org/obo/GAZ_00006949"/>
        <obo:IAO_0000115>A South Pacific Ocean atoll located in the Tokelau Group. Sits atop the Fakaofo Seamount.</obo:IAO_0000115>
        <oboInOwl:hasOBONamespace>GAZ</oboInOwl:hasOBONamespace>
        <oboInOwl:id>GAZ:00006951</oboInOwl:id>
        <rdfs:label>Fakaofo Atoll</rdfs:label>
    </owl:NamedIndividual>
    


    <!-- http://purl.obolibrary.org/obo/GAZ_00007126 -->

    <owl:NamedIndividual rdf:about="http://purl.obolibrary.org/obo/GAZ_00007126">
        <obo:RO_0001025 rdf:resource="http://purl.obolibrary.org/obo/GAZ_00000469"/>
        <obo:IAO_0000115>An archipelago that is located roughly 800 km east of Christchurch, New Zealand. They cover a total of 966 km2, almost all of which is in the two main islands, Chatham Island and Pitt Island.</obo:IAO_0000115>
        <oboInOwl:hasOBONamespace>GAZ</oboInOwl:hasOBONamespace>
        <oboInOwl:id>GAZ:00007126</oboInOwl:id>
        <rdfs:label>Chatham Islands</rdfs:label>
    </owl:NamedIndividual>
    


    <!-- http://purl.obolibrary.org/obo/GAZ_00007139 -->

    <owl:NamedIndividual rdf:about="http://purl.obolibrary.org/obo/GAZ_00007139">
        <obo:RO_0001025 rdf:resource="http://purl.obolibrary.org/obo/GAZ_00000469"/>
        <obo:IAO_0000115>An island volcanic arc in the South Pacific Ocean. The islands have been part of New Zealand since 1887.</obo:IAO_0000115>
        <oboInOwl:hasOBONamespace>GAZ</oboInOwl:hasOBONamespace>
        <oboInOwl:id>GAZ:00007139</oboInOwl:id>
        <rdfs:label>Kermadec Islands</rdfs:label>
    </owl:NamedIndividual>
    


    <!-- http://purl.obolibrary.org/obo/GAZ_00007140 -->

    <owl:NamedIndividual rdf:about="http://purl.obolibrary.org/obo/GAZ_00007140">
        <obo:RO_0001025 rdf:resource="http://purl.obolibrary.org/obo/GAZ_00007139"/>
        <obo:IAO_0000115>Rocks located 80 km SSE of Curtis Island.</obo:IAO_0000115>
        <oboInOwl:hasOBONamespace>GAZ</oboInOwl:hasOBONamespace>
        <oboInOwl:id>GAZ:00007140</oboInOwl:id>
        <rdfs:label>L&apos;Esperance Rock</rdfs:label>
    </owl:NamedIndividual>
    


    <!-- http://purl.obolibrary.org/obo/GAZ_00007141 -->

    <owl:NamedIndividual rdf:about="http://purl.obolibrary.org/obo/GAZ_00007141">
        <obo:RO_0001025 rdf:resource="http://purl.obolibrary.org/obo/GAZ_00007139"/>
        <obo:IAO_0000115>With nearby Cheeseman Island, the uplifted portion of a submarine volcano astride the Kermadec Ridge. The age of the small islands is considered to be Pleistocene, and rocks consist dominantly, if not entirely, of andesitic pyroclastic-flow deposits (Lloyd, 1992). Curtis Island, only 500 x 800 m in diameter and 137-m high, contains a large, fumarolically active crater whose floor is only 10 m above sea level. Reports of possible historical eruptions probably represent increased thermal activity. Geologic studies have documented a remarkable uplift of 18 m of Curtis Island during the past 200 years, with 7 m of uplift occurring between 1929 and 1964 (Doyle et al., 1979). An active submarine magmatic or solfataric vent is believed to exist near Curtis Island, but its activity cannot unequivocally be associated with Curtis volcano (Lloyd, 1992).</obo:IAO_0000115>
        <oboInOwl:hasOBONamespace>GAZ</oboInOwl:hasOBONamespace>
        <oboInOwl:id>GAZ:00007141</oboInOwl:id>
        <rdfs:label>Curtis Island</rdfs:label>
    </owl:NamedIndividual>
    


    <!-- http://purl.obolibrary.org/obo/GAZ_00007142 -->

    <owl:NamedIndividual rdf:about="http://purl.obolibrary.org/obo/GAZ_00007142">
        <obo:RO_0001025 rdf:resource="http://purl.obolibrary.org/obo/GAZ_00007139"/>
        <obo:IAO_0000115>A remnant of the rim of a large submarine caldera centered 8 km to the NW. The 3 km wide island consists of a low, gently sloping surface of rhyolitic pumice from the caldera-forming eruption truncated by steep cliffs formed of underlying basaltic lava flows. The pre-caldera Macauley volcano consisted of two generations of shield volcanoes separated by a period of growth of a pyroclastic cone. Eruption of the voluminous Sandy Bay Tuff about 6300 years ago truncated the NW side of the Annexation shield volcano and formed a 12 km wide, 1.1 km deep caldera during one of the largest eruptions identified in the SW Pacific. Following formation of the caldera and substantial marine erosion, a partly submarine and partly subaerial eruption centered about 2 km north of present-day Macauley Island produced basaltic scoriae and lava flows.</obo:IAO_0000115>
        <oboInOwl:hasOBONamespace>GAZ</oboInOwl:hasOBONamespace>
        <oboInOwl:id>GAZ:00007142</oboInOwl:id>
        <rdfs:label>Macauley Island</rdfs:label>
    </owl:NamedIndividual>
    


    <!-- http://purl.obolibrary.org/obo/GAZ_00007143 -->

    <owl:NamedIndividual rdf:about="http://purl.obolibrary.org/obo/GAZ_00007143">
        <obo:RO_0001025 rdf:resource="http://purl.obolibrary.org/obo/GAZ_00053816"/>
        <obo:IAO_0000115>The largest and northernmost of the Kermadec Islands, located 900 km SSW of &apos;Ata Island of Tonga and 1100 km NNE of New Zealand&apos;s North Island. A stratovolcanic island. Two Holocene calderas are found at Raoul. The older caldera cuts the center of Raoul Island and is about 2.5 x 3.5 km wide. Denham caldera, formed during a major dacitic explosive eruption about 2200 years ago, truncated the western side of the island and is 6.5 x 4 km wide. Its long axis is parallel to the tectonic fabric of the Havre Trough that lies west of the volcanic arc. Historical eruptions at Raoul during the 19th and 20th centuries have sometimes occurred simultaneously from both calderas, and have consisted of small-to-moderate phreatic eruptions, some of which formed ephemeral islands in Denham caldera. A 240 m high unnamed submarine cone, one of several located along a fissure on the lower NNE flank of Raoul volcano, has also erupted during historical time, and satellitic vents at Raoul are concentrated along two parallel NNE-trending lineaments.</obo:IAO_0000115>
        <oboInOwl:hasOBONamespace>GAZ</oboInOwl:hasOBONamespace>
        <oboInOwl:id>GAZ:00007143</oboInOwl:id>
        <rdfs:label>Raoul Island</rdfs:label>
    </owl:NamedIndividual>
    


    <!-- http://purl.obolibrary.org/obo/GAZ_00007172 -->

    <owl:NamedIndividual rdf:about="http://purl.obolibrary.org/obo/GAZ_00007172">
        <obo:RO_0001025 rdf:resource="http://purl.obolibrary.org/obo/GAZ_00000469"/>
        <obo:IAO_0000115>A group of volcanic islands to the south of, and territorially part of, New Zealand. The position of the Antipodes Islands relative to New Zealand, and other outlying islands. The position of the Antipodes Islands relative to New Zealand, and other outlying islands. They lie 650 km to the southeast of Stewart Island/Rakiura. The group consists of one main island of 60 km2 area, Bollons Island of 2 km2 to the north, and numerous small islets and stacks. The highest point is Mount Galloway (402 m), which is also the group&apos;s most recently active volcano.</obo:IAO_0000115>
        <oboInOwl:hasOBONamespace>GAZ</oboInOwl:hasOBONamespace>
        <oboInOwl:id>GAZ:00007172</oboInOwl:id>
        <rdfs:label>Antipodes Islands</rdfs:label>
    </owl:NamedIndividual>
    


    <!-- http://purl.obolibrary.org/obo/GAZ_00007173 -->

    <owl:NamedIndividual rdf:about="http://purl.obolibrary.org/obo/GAZ_00007173">
        <obo:RO_0001025 rdf:resource="http://purl.obolibrary.org/obo/GAZ_00000469"/>
        <obo:IAO_0000115>An archipelago of the New Zealand Sub-Antarctic Islands and include the following: Auckland Island, Adams Island, Enderby Island, Disappointment Island, Ewing Island, Dundas Island and Green Island. They lie 465 km from the South Island port of Bluff.</obo:IAO_0000115>
        <oboInOwl:hasOBONamespace>GAZ</oboInOwl:hasOBONamespace>
        <oboInOwl:id>GAZ:00007173</oboInOwl:id>
        <rdfs:label>Auckland Islands</rdfs:label>
    </owl:NamedIndividual>
    


    <!-- http://purl.obolibrary.org/obo/GAZ_00007174 -->

    <owl:NamedIndividual rdf:about="http://purl.obolibrary.org/obo/GAZ_00007174">
        <obo:RO_0001025 rdf:resource="http://purl.obolibrary.org/obo/GAZ_00000469"/>
        <obo:IAO_0000115>A small group of 13 islets and numerous rocks in the south Pacific Ocean which are territorially part of New Zealand.</obo:IAO_0000115>
        <oboInOwl:hasOBONamespace>GAZ</oboInOwl:hasOBONamespace>
        <oboInOwl:id>GAZ:00007174</oboInOwl:id>
        <rdfs:label>Bounty Islands</rdfs:label>
    </owl:NamedIndividual>
    


    <!-- http://purl.obolibrary.org/obo/GAZ_00007175 -->

    <owl:NamedIndividual rdf:about="http://purl.obolibrary.org/obo/GAZ_00007175">
        <obo:RO_0001025 rdf:resource="http://purl.obolibrary.org/obo/GAZ_00000469"/>
        <obo:IAO_0000115>A group of sub-Antarctic islands, belonging to New Zealand. The Campbell Island group consists of one big island, Campbell Island, and several much smaller islets like Dent Island, Folly Island (or Folly Islands) and Jacquemart Island.</obo:IAO_0000115>
        <oboInOwl:hasOBONamespace>GAZ</oboInOwl:hasOBONamespace>
        <oboInOwl:id>GAZ:00007175</oboInOwl:id>
        <rdfs:label>Campbell Islands</rdfs:label>
    </owl:NamedIndividual>
    


    <!-- http://purl.obolibrary.org/obo/GAZ_00007176 -->

    <owl:NamedIndividual rdf:about="http://purl.obolibrary.org/obo/GAZ_00007176">
        <rdf:type rdf:resource="http://purl.obolibrary.org/obo/ENVO_00000220"/>
        <obo:RO_0001025 rdf:resource="http://purl.obolibrary.org/obo/GAZ_00008572"/>
        <obo:IAO_0000115>A small island group approximately 200 km south of New Zealand&apos;s South Island. The Snares consist of the main island North East Island and the smaller Broughton Island as well as the somewhat isolated Western Chain Islands approx 5 km to the WSW. As a group of islands, the Snares cover a total of approximately 3.5 km2.</obo:IAO_0000115>
        <oboInOwl:hasOBONamespace>GAZ</oboInOwl:hasOBONamespace>
        <oboInOwl:id>GAZ:00007176</oboInOwl:id>
        <rdfs:label>The Snares</rdfs:label>
    </owl:NamedIndividual>
    


    <!-- http://purl.obolibrary.org/obo/GAZ_00007177 -->

    <owl:NamedIndividual rdf:about="http://purl.obolibrary.org/obo/GAZ_00007177">
        <obo:RO_0001025 rdf:resource="http://purl.obolibrary.org/obo/GAZ_00047005"/>
        <obo:IAO_0000115>A small chain of uninhabited volcanic islets lying close to the western end of the Foveaux Strait in southern New Zealand. They lie some 38 km south of Prices Point on the southern coast of South Island, New Zealand, close where Lake Hakapoua drains through Big River to the Pacific Ocean due west of Te Waewae Bay, and 64 km WNW of the Putatara (Rugged) Point in the northwest of Stewart Island, or 56 km from Codfish Island west of Stewart Island. They measure about 0.7 km2 in area. Administratively, they are part of Southland District.</obo:IAO_0000115>
        <oboInOwl:hasOBONamespace>GAZ</oboInOwl:hasOBONamespace>
        <oboInOwl:id>GAZ:00007177</oboInOwl:id>
        <rdfs:label>Solander Islands</rdfs:label>
    </owl:NamedIndividual>
    


    <!-- http://purl.obolibrary.org/obo/GAZ_00007178 -->

    <owl:NamedIndividual rdf:about="http://purl.obolibrary.org/obo/GAZ_00007178">
        <obo:RO_0001025 rdf:resource="http://purl.obolibrary.org/obo/GAZ_00000469"/>
        <obo:IAO_0000115>A group of 13 islands about 55 km northwest of Cape Reinga, the northernmost point of the North Island of New Zealand, where the South Pacific Ocean and Tasman Sea converge.</obo:IAO_0000115>
        <oboInOwl:hasOBONamespace>GAZ</oboInOwl:hasOBONamespace>
        <oboInOwl:id>GAZ:00007178</oboInOwl:id>
        <rdfs:label>Three Kings Islands</rdfs:label>
    </owl:NamedIndividual>
    


    <!-- http://purl.obolibrary.org/obo/GAZ_00007355 -->

    <owl:NamedIndividual rdf:about="http://purl.obolibrary.org/obo/GAZ_00007355">
        <obo:RO_0001025 rdf:resource="http://purl.obolibrary.org/obo/GAZ_00004773"/>
        <oboInOwl:hasOBONamespace>GAZ</oboInOwl:hasOBONamespace>
        <oboInOwl:id>GAZ:00007355</oboInOwl:id>
        <rdfs:label>Milson</rdfs:label>
    </owl:NamedIndividual>
    


    <!-- http://purl.obolibrary.org/obo/GAZ_00007530 -->

    <owl:NamedIndividual rdf:about="http://purl.obolibrary.org/obo/GAZ_00007530">
        <obo:RO_0001025 rdf:resource="http://purl.obolibrary.org/obo/GAZ_00004765"/>
        <oboInOwl:hasOBONamespace>GAZ</oboInOwl:hasOBONamespace>
        <oboInOwl:id>GAZ:00007530</oboInOwl:id>
        <rdfs:label>Waimangu Valley</rdfs:label>
    </owl:NamedIndividual>
    


    <!-- http://purl.obolibrary.org/obo/GAZ_00007531 -->

    <owl:NamedIndividual rdf:about="http://purl.obolibrary.org/obo/GAZ_00007531">
        <obo:RO_0001025 rdf:resource="http://purl.obolibrary.org/obo/GAZ_00007530"/>
        <obo:IAO_0000115>A hot spring.</obo:IAO_0000115>
        <oboInOwl:hasOBONamespace>GAZ</oboInOwl:hasOBONamespace>
        <oboInOwl:id>GAZ:00007531</oboInOwl:id>
        <rdfs:label>The Clamshell</rdfs:label>
    </owl:NamedIndividual>
    


    <!-- http://purl.obolibrary.org/obo/GAZ_00007545 -->

    <owl:NamedIndividual rdf:about="http://purl.obolibrary.org/obo/GAZ_00007545">
        <obo:RO_0001025 rdf:resource="http://purl.obolibrary.org/obo/GAZ_00029953"/>
        <obo:RO_0001025 rdf:resource="http://purl.obolibrary.org/obo/GAZ_00051945"/>
        <obo:IAO_0000115>A national park located in the central North Island.</obo:IAO_0000115>
        <oboInOwl:hasOBONamespace>GAZ</oboInOwl:hasOBONamespace>
        <oboInOwl:id>GAZ:00007545</oboInOwl:id>
        <rdfs:label>Tongariro National Park</rdfs:label>
    </owl:NamedIndividual>
    


    <!-- http://purl.obolibrary.org/obo/GAZ_00007723 -->

    <owl:NamedIndividual rdf:about="http://purl.obolibrary.org/obo/GAZ_00007723">
        <obo:RO_0001025 rdf:resource="http://purl.obolibrary.org/obo/GAZ_00004765"/>
    </owl:NamedIndividual>
    


    <!-- http://purl.obolibrary.org/obo/GAZ_00007724 -->

    <owl:NamedIndividual rdf:about="http://purl.obolibrary.org/obo/GAZ_00007724">
        <obo:RO_0001025 rdf:resource="http://purl.obolibrary.org/obo/GAZ_00051944"/>
    </owl:NamedIndividual>
    


    <!-- http://purl.obolibrary.org/obo/GAZ_00008133 -->

    <owl:NamedIndividual rdf:about="http://purl.obolibrary.org/obo/GAZ_00008133">
        <obo:RO_0001025 rdf:resource="http://purl.obolibrary.org/obo/GAZ_00007724"/>
        <oboInOwl:hasOBONamespace>GAZ</oboInOwl:hasOBONamespace>
        <oboInOwl:id>GAZ:00008133</oboInOwl:id>
        <rdfs:label>Kuirau Park</rdfs:label>
    </owl:NamedIndividual>
    


    <!-- http://purl.obolibrary.org/obo/GAZ_00008392 -->

    <owl:NamedIndividual rdf:about="http://purl.obolibrary.org/obo/GAZ_00008392">
        <obo:RO_0001025 rdf:resource="http://purl.obolibrary.org/obo/GAZ_00009534"/>
        <oboInOwl:hasOBONamespace>GAZ</oboInOwl:hasOBONamespace>
        <oboInOwl:id>GAZ:00008392</oboInOwl:id>
        <rdfs:label>South Auckland</rdfs:label>
    </owl:NamedIndividual>
    


    <!-- http://purl.obolibrary.org/obo/GAZ_00008560 -->

    <owl:NamedIndividual rdf:about="http://purl.obolibrary.org/obo/GAZ_00008560">
        <obo:RO_0001025 rdf:resource="http://purl.obolibrary.org/obo/GAZ_00004764"/>
        <oboInOwl:hasOBONamespace>GAZ</oboInOwl:hasOBONamespace>
        <oboInOwl:id>GAZ:00008560</oboInOwl:id>
        <rdfs:label>Nelson District</rdfs:label>
    </owl:NamedIndividual>
    


    <!-- http://purl.obolibrary.org/obo/GAZ_00008561 -->

    <owl:NamedIndividual rdf:about="http://purl.obolibrary.org/obo/GAZ_00008561">
        <obo:RO_0001025 rdf:resource="http://purl.obolibrary.org/obo/GAZ_00004781"/>
    </owl:NamedIndividual>
    


    <!-- http://purl.obolibrary.org/obo/GAZ_00008562 -->

    <owl:NamedIndividual rdf:about="http://purl.obolibrary.org/obo/GAZ_00008562">
        <obo:RO_0001025 rdf:resource="http://purl.obolibrary.org/obo/GAZ_00004764"/>
    </owl:NamedIndividual>
    


    <!-- http://purl.obolibrary.org/obo/GAZ_00008563 -->

    <owl:NamedIndividual rdf:about="http://purl.obolibrary.org/obo/GAZ_00008563">
        <obo:RO_0001025 rdf:resource="http://purl.obolibrary.org/obo/GAZ_00004764"/>
        <obo:IAO_0000115>A region of New Zealand. It borders with the West Coast Region, Marlborough Region and the Nelson Region. It is bounded to the west by the Matiri Ranges, Tasman Mountains and the Tasman Sea. To the north Tasman and Golden Bays form its seaward edge, and the eastern boundary extends to the edge of Nelson city, and includes part of the Spencer Mountains and the Saint Arnaud and Richmond Ranges. The Victoria Ranges form Tasman&apos;s southern boundary and the district&apos;s highest point is Mt Owen, at 1,875 metres.</obo:IAO_0000115>
        <oboInOwl:hasOBONamespace>GAZ</oboInOwl:hasOBONamespace>
        <oboInOwl:id>GAZ:00008563</oboInOwl:id>
        <rdfs:label>Tasman District</rdfs:label>
    </owl:NamedIndividual>
    


    <!-- http://purl.obolibrary.org/obo/GAZ_00008564 -->

    <owl:NamedIndividual rdf:about="http://purl.obolibrary.org/obo/GAZ_00008564">
        <obo:RO_0001025 rdf:resource="http://purl.obolibrary.org/obo/GAZ_00004765"/>
    </owl:NamedIndividual>
    


    <!-- http://purl.obolibrary.org/obo/GAZ_00008565 -->

    <owl:NamedIndividual rdf:about="http://purl.obolibrary.org/obo/GAZ_00008565">
        <obo:RO_0001025 rdf:resource="http://purl.obolibrary.org/obo/GAZ_00004765"/>
        <obo:RO_0001025 rdf:resource="http://purl.obolibrary.org/obo/GAZ_00010255"/>
    </owl:NamedIndividual>
    


    <!-- http://purl.obolibrary.org/obo/GAZ_00008567 -->

    <owl:NamedIndividual rdf:about="http://purl.obolibrary.org/obo/GAZ_00008567">
        <obo:RO_0001025 rdf:resource="http://purl.obolibrary.org/obo/GAZ_00004772"/>
        <obo:RO_0001025 rdf:resource="http://purl.obolibrary.org/obo/GAZ_00008565"/>
        <oboInOwl:hasOBONamespace>GAZ</oboInOwl:hasOBONamespace>
        <oboInOwl:id>GAZ:00008567</oboInOwl:id>
        <rdfs:label>Tararua District</rdfs:label>
    </owl:NamedIndividual>
    


    <!-- http://purl.obolibrary.org/obo/GAZ_00008568 -->

    <owl:NamedIndividual rdf:about="http://purl.obolibrary.org/obo/GAZ_00008568">
        <obo:RO_0001025 rdf:resource="http://purl.obolibrary.org/obo/GAZ_00004764"/>
    </owl:NamedIndividual>
    


    <!-- http://purl.obolibrary.org/obo/GAZ_00008569 -->

    <owl:NamedIndividual rdf:about="http://purl.obolibrary.org/obo/GAZ_00008569">
        <obo:RO_0001025 rdf:resource="http://purl.obolibrary.org/obo/GAZ_00004765"/>
    </owl:NamedIndividual>
    


    <!-- http://purl.obolibrary.org/obo/GAZ_00008570 -->

    <owl:NamedIndividual rdf:about="http://purl.obolibrary.org/obo/GAZ_00008570">
        <obo:RO_0001025 rdf:resource="http://purl.obolibrary.org/obo/GAZ_00009537"/>
    </owl:NamedIndividual>
    


    <!-- http://purl.obolibrary.org/obo/GAZ_00008571 -->

    <owl:NamedIndividual rdf:about="http://purl.obolibrary.org/obo/GAZ_00008571">
        <obo:RO_0001025 rdf:resource="http://purl.obolibrary.org/obo/GAZ_00008570"/>
    </owl:NamedIndividual>
    


    <!-- http://purl.obolibrary.org/obo/GAZ_00008572 -->

    <owl:NamedIndividual rdf:about="http://purl.obolibrary.org/obo/GAZ_00008572">
        <obo:RO_0001025 rdf:resource="http://purl.obolibrary.org/obo/GAZ_00004764"/>
    </owl:NamedIndividual>
    


    <!-- http://purl.obolibrary.org/obo/GAZ_00008578 -->

    <owl:NamedIndividual rdf:about="http://purl.obolibrary.org/obo/GAZ_00008578">
        <obo:RO_0001025 rdf:resource="http://purl.obolibrary.org/obo/GAZ_00142240"/>
        <obo:IAO_0000115>A crater lake.</obo:IAO_0000115>
        <oboInOwl:hasOBONamespace>GAZ</oboInOwl:hasOBONamespace>
        <oboInOwl:id>GAZ:00008578</oboInOwl:id>
        <rdfs:label>Green Lake</rdfs:label>
    </owl:NamedIndividual>
    


    <!-- http://purl.obolibrary.org/obo/GAZ_00008752 -->

    <owl:NamedIndividual rdf:about="http://purl.obolibrary.org/obo/GAZ_00008752">
        <obo:RO_0001025 rdf:resource="http://purl.obolibrary.org/obo/GAZ_00007724"/>
        <obo:RO_0001025 rdf:resource="http://purl.obolibrary.org/obo/GAZ_00051945"/>
        <obo:IAO_0000115>A geothermal area within Rotorua city in the Taupo Volcanic Zone of New Zealand. Whakawerawera has some 500 pools, most of which are alkaline chloride hot springs, and at least 65 geyser vents, each with their own name. Seven geysers are currently active. The most famous, Pohutu Geyser, meaning big splash or explosion, can erupt up to 30 m, usually every hour.</obo:IAO_0000115>
        <oboInOwl:hasOBONamespace>GAZ</oboInOwl:hasOBONamespace>
        <oboInOwl:id>GAZ:00008752</oboInOwl:id>
        <rdfs:label>Whakarewarewa</rdfs:label>
    </owl:NamedIndividual>
    


    <!-- http://purl.obolibrary.org/obo/GAZ_00009534 -->

    <owl:NamedIndividual rdf:about="http://purl.obolibrary.org/obo/GAZ_00009534">
        <obo:RO_0001025 rdf:resource="http://purl.obolibrary.org/obo/GAZ_00004760"/>
    </owl:NamedIndividual>
    


    <!-- http://purl.obolibrary.org/obo/GAZ_00009535 -->

    <owl:NamedIndividual rdf:about="http://purl.obolibrary.org/obo/GAZ_00009535">
        <obo:RO_0001025 rdf:resource="http://purl.obolibrary.org/obo/GAZ_00004781"/>
        <obo:RO_0001025 rdf:resource="http://purl.obolibrary.org/obo/GAZ_00007723"/>
        <oboInOwl:hasOBONamespace>GAZ</oboInOwl:hasOBONamespace>
        <oboInOwl:id>GAZ:00009535</oboInOwl:id>
        <rdfs:label>Rotorua District</rdfs:label>
    </owl:NamedIndividual>
    


    <!-- http://purl.obolibrary.org/obo/GAZ_00009536 -->

    <owl:NamedIndividual rdf:about="http://purl.obolibrary.org/obo/GAZ_00009536">
        <obo:RO_0001025 rdf:resource="http://purl.obolibrary.org/obo/GAZ_00004772"/>
        <oboInOwl:hasOBONamespace>GAZ</oboInOwl:hasOBONamespace>
        <oboInOwl:id>GAZ:00009536</oboInOwl:id>
        <rdfs:label>Stratford District</rdfs:label>
    </owl:NamedIndividual>
    


    <!-- http://purl.obolibrary.org/obo/GAZ_00009537 -->

    <owl:NamedIndividual rdf:about="http://purl.obolibrary.org/obo/GAZ_00009537">
        <obo:RO_0001025 rdf:resource="http://purl.obolibrary.org/obo/GAZ_00008569"/>
        <oboInOwl:hasOBONamespace>GAZ</oboInOwl:hasOBONamespace>
        <oboInOwl:id>GAZ:00009537</oboInOwl:id>
        <rdfs:label>Whangarei District</rdfs:label>
    </owl:NamedIndividual>
    


    <!-- http://purl.obolibrary.org/obo/GAZ_00009539 -->

    <owl:NamedIndividual rdf:about="http://purl.obolibrary.org/obo/GAZ_00009539">
        <obo:RO_0001025 rdf:resource="http://purl.obolibrary.org/obo/GAZ_00004767"/>
        <oboInOwl:hasOBONamespace>GAZ</oboInOwl:hasOBONamespace>
        <oboInOwl:id>GAZ:00009539</oboInOwl:id>
        <rdfs:label>Central Otago District</rdfs:label>
    </owl:NamedIndividual>
    


    <!-- http://purl.obolibrary.org/obo/GAZ_00009541 -->

    <owl:NamedIndividual rdf:about="http://purl.obolibrary.org/obo/GAZ_00009541">
        <obo:RO_0001025 rdf:resource="http://purl.obolibrary.org/obo/GAZ_00004781"/>
        <obo:RO_0001025 rdf:resource="http://purl.obolibrary.org/obo/GAZ_00007723"/>
        <obo:RO_0001025 rdf:resource="http://purl.obolibrary.org/obo/GAZ_00010256"/>
        <oboInOwl:hasOBONamespace>GAZ</oboInOwl:hasOBONamespace>
        <oboInOwl:id>GAZ:00009541</oboInOwl:id>
        <rdfs:label>Taupo District</rdfs:label>
    </owl:NamedIndividual>
    


    <!-- http://purl.obolibrary.org/obo/GAZ_00009560 -->

    <owl:NamedIndividual rdf:about="http://purl.obolibrary.org/obo/GAZ_00009560">
        <obo:RO_0001025 rdf:resource="http://purl.obolibrary.org/obo/GAZ_00006950"/>
        <oboInOwl:hasOBONamespace>GAZ</oboInOwl:hasOBONamespace>
        <oboInOwl:id>GAZ:00009560</oboInOwl:id>
        <rdfs:label>Nukunonu Community</rdfs:label>
    </owl:NamedIndividual>
    


    <!-- http://purl.obolibrary.org/obo/GAZ_00009561 -->

    <owl:NamedIndividual rdf:about="http://purl.obolibrary.org/obo/GAZ_00009561">
        <obo:RO_0001025 rdf:resource="http://purl.obolibrary.org/obo/GAZ_00006951"/>
        <oboInOwl:hasOBONamespace>GAZ</oboInOwl:hasOBONamespace>
        <oboInOwl:id>GAZ:00009561</oboInOwl:id>
        <rdfs:label>Fakaofo Community</rdfs:label>
    </owl:NamedIndividual>
    


    <!-- http://purl.obolibrary.org/obo/GAZ_00009562 -->

    <owl:NamedIndividual rdf:about="http://purl.obolibrary.org/obo/GAZ_00009562">
        <obo:RO_0001025 rdf:resource="http://purl.obolibrary.org/obo/GAZ_00142022"/>
        <oboInOwl:hasOBONamespace>GAZ</oboInOwl:hasOBONamespace>
        <oboInOwl:id>GAZ:00009562</oboInOwl:id>
        <rdfs:label>Atafu Community</rdfs:label>
    </owl:NamedIndividual>
    


    <!-- http://purl.obolibrary.org/obo/GAZ_00009760 -->

    <owl:NamedIndividual rdf:about="http://purl.obolibrary.org/obo/GAZ_00009760">
        <obo:RO_0001025 rdf:resource="http://purl.obolibrary.org/obo/GAZ_00008565"/>
    </owl:NamedIndividual>
    


    <!-- http://purl.obolibrary.org/obo/GAZ_00009762 -->

    <owl:NamedIndividual rdf:about="http://purl.obolibrary.org/obo/GAZ_00009762">
        <obo:RO_0001025 rdf:resource="http://purl.obolibrary.org/obo/GAZ_00008565"/>
    </owl:NamedIndividual>
    


    <!-- http://purl.obolibrary.org/obo/GAZ_00009763 -->

    <owl:NamedIndividual rdf:about="http://purl.obolibrary.org/obo/GAZ_00009763">
        <obo:RO_0001025 rdf:resource="http://purl.obolibrary.org/obo/GAZ_00008565"/>
    </owl:NamedIndividual>
    


    <!-- http://purl.obolibrary.org/obo/GAZ_00009775 -->

    <owl:NamedIndividual rdf:about="http://purl.obolibrary.org/obo/GAZ_00009775">
        <rdf:type rdf:resource="http://purl.obolibrary.org/obo/ENVO_00000004"/>
        <obo:RO_0001025 rdf:resource="http://purl.obolibrary.org/obo/GAZ_00004772"/>
        <obo:IAO_0000115>A district on the west coast of the North Island of New Zealand. It is part of the Manawatu-Wanganui region. Wanganui District Council resulted from amalgamation of Wanganui and Waitotara county councils and Wanganui City Council.</obo:IAO_0000115>
        <oboInOwl:hasOBONamespace>GAZ</oboInOwl:hasOBONamespace>
        <oboInOwl:id>GAZ:00009775</oboInOwl:id>
        <rdfs:label>Wanganui District</rdfs:label>
    </owl:NamedIndividual>
    


    <!-- http://purl.obolibrary.org/obo/GAZ_00009776 -->

    <owl:NamedIndividual rdf:about="http://purl.obolibrary.org/obo/GAZ_00009776">
        <obo:RO_0001025 rdf:resource="http://purl.obolibrary.org/obo/GAZ_00009775"/>
    </owl:NamedIndividual>
    


    <!-- http://purl.obolibrary.org/obo/GAZ_00010240 -->

    <owl:NamedIndividual rdf:about="http://purl.obolibrary.org/obo/GAZ_00010240">
        <obo:RO_0001025 rdf:resource="http://purl.obolibrary.org/obo/GAZ_00007723"/>
    </owl:NamedIndividual>
    


    <!-- http://purl.obolibrary.org/obo/GAZ_00010241 -->

    <owl:NamedIndividual rdf:about="http://purl.obolibrary.org/obo/GAZ_00010241">
        <obo:RO_0001025 rdf:resource="http://purl.obolibrary.org/obo/GAZ_00012588"/>
    </owl:NamedIndividual>
    


    <!-- http://purl.obolibrary.org/obo/GAZ_00010242 -->

    <owl:NamedIndividual rdf:about="http://purl.obolibrary.org/obo/GAZ_00010242">
        <obo:RO_0001025 rdf:resource="http://purl.obolibrary.org/obo/GAZ_00008562"/>
        <oboInOwl:hasOBONamespace>GAZ</oboInOwl:hasOBONamespace>
        <oboInOwl:id>GAZ:00010242</oboInOwl:id>
        <rdfs:label>Timaru District</rdfs:label>
    </owl:NamedIndividual>
    


    <!-- http://purl.obolibrary.org/obo/GAZ_00010243 -->

    <owl:NamedIndividual rdf:about="http://purl.obolibrary.org/obo/GAZ_00010243">
        <obo:RO_0001025 rdf:resource="http://purl.obolibrary.org/obo/GAZ_00008562"/>
        <oboInOwl:hasOBONamespace>GAZ</oboInOwl:hasOBONamespace>
        <oboInOwl:id>GAZ:00010243</oboInOwl:id>
        <rdfs:label>Selwyn District</rdfs:label>
    </owl:NamedIndividual>
    


    <!-- http://purl.obolibrary.org/obo/GAZ_00010244 -->

    <owl:NamedIndividual rdf:about="http://purl.obolibrary.org/obo/GAZ_00010244">
        <obo:RO_0001025 rdf:resource="http://purl.obolibrary.org/obo/GAZ_00008562"/>
        <oboInOwl:hasOBONamespace>GAZ</oboInOwl:hasOBONamespace>
        <oboInOwl:id>GAZ:00010244</oboInOwl:id>
        <rdfs:label>Ashburton District</rdfs:label>
    </owl:NamedIndividual>
    


    <!-- http://purl.obolibrary.org/obo/GAZ_00010245 -->

    <owl:NamedIndividual rdf:about="http://purl.obolibrary.org/obo/GAZ_00010245">
        <obo:RO_0001025 rdf:resource="http://purl.obolibrary.org/obo/GAZ_00010244"/>
    </owl:NamedIndividual>
    


    <!-- http://purl.obolibrary.org/obo/GAZ_00010246 -->

    <owl:NamedIndividual rdf:about="http://purl.obolibrary.org/obo/GAZ_00010246">
        <obo:RO_0001025 rdf:resource="http://purl.obolibrary.org/obo/GAZ_00008562"/>
    </owl:NamedIndividual>
    


    <!-- http://purl.obolibrary.org/obo/GAZ_00010247 -->

    <owl:NamedIndividual rdf:about="http://purl.obolibrary.org/obo/GAZ_00010247">
        <obo:RO_0001025 rdf:resource="http://purl.obolibrary.org/obo/GAZ_00010242"/>
    </owl:NamedIndividual>
    


    <!-- http://purl.obolibrary.org/obo/GAZ_00010248 -->

    <owl:NamedIndividual rdf:about="http://purl.obolibrary.org/obo/GAZ_00010248">
        <obo:RO_0001025 rdf:resource="http://purl.obolibrary.org/obo/GAZ_00004765"/>
        <obo:IAO_0000115>A unitary authority in New Zealand, being both a region and a district. It is located in the northeastern corner of the North Island.</obo:IAO_0000115>
        <oboInOwl:hasOBONamespace>GAZ</oboInOwl:hasOBONamespace>
        <oboInOwl:id>GAZ:00010248</oboInOwl:id>
        <rdfs:label>Gisborne District</rdfs:label>
    </owl:NamedIndividual>
    


    <!-- http://purl.obolibrary.org/obo/GAZ_00010249 -->

    <owl:NamedIndividual rdf:about="http://purl.obolibrary.org/obo/GAZ_00010249">
        <obo:RO_0001025 rdf:resource="http://purl.obolibrary.org/obo/GAZ_00010248"/>
        <oboInOwl:hasOBONamespace>GAZ</oboInOwl:hasOBONamespace>
        <oboInOwl:id>GAZ:00010249</oboInOwl:id>
        <rdfs:label>Tairawhiti</rdfs:label>
    </owl:NamedIndividual>
    


    <!-- http://purl.obolibrary.org/obo/GAZ_00010250 -->

    <owl:NamedIndividual rdf:about="http://purl.obolibrary.org/obo/GAZ_00010250">
        <obo:RO_0001025 rdf:resource="http://purl.obolibrary.org/obo/GAZ_00008568"/>
    </owl:NamedIndividual>
    


    <!-- http://purl.obolibrary.org/obo/GAZ_00010251 -->

    <owl:NamedIndividual rdf:about="http://purl.obolibrary.org/obo/GAZ_00010251">
        <obo:RO_0001025 rdf:resource="http://purl.obolibrary.org/obo/GAZ_00008560"/>
    </owl:NamedIndividual>
    


    <!-- http://purl.obolibrary.org/obo/GAZ_00010253 -->

    <owl:NamedIndividual rdf:about="http://purl.obolibrary.org/obo/GAZ_00010253">
        <obo:RO_0001025 rdf:resource="http://purl.obolibrary.org/obo/GAZ_00004768"/>
        <obo:IAO_0000115>The main port of the city of Dunedin, New Zealand.</obo:IAO_0000115>
        <oboInOwl:hasOBONamespace>GAZ</oboInOwl:hasOBONamespace>
        <oboInOwl:id>GAZ:00010253</oboInOwl:id>
        <rdfs:label>Port Chalmers</rdfs:label>
    </owl:NamedIndividual>
    


    <!-- http://purl.obolibrary.org/obo/GAZ_00010254 -->

    <owl:NamedIndividual rdf:about="http://purl.obolibrary.org/obo/GAZ_00010254">
        <obo:RO_0001025 rdf:resource="http://purl.obolibrary.org/obo/GAZ_00008572"/>
    </owl:NamedIndividual>
    


    <!-- http://purl.obolibrary.org/obo/GAZ_00010255 -->

    <owl:NamedIndividual rdf:about="http://purl.obolibrary.org/obo/GAZ_00010255">
        <obo:RO_0001025 rdf:resource="http://purl.obolibrary.org/obo/GAZ_00004765"/>
        <obo:IAO_0000115>A geographical region of New Zealand. It occupies the south-eastern corner of the North Island, east of metropolitan Wellington and south-west of the Hawke&apos;s Bay region. The area is divided between the local government regions of Wellington, Manawatu-Wanganui, and Hawke&apos;s Bay. The area south of Mt. Bruce is in the Greater Wellington Region. It contains the Masterton, Carterton and South Wairarapa Districts. It is separated from Upper Hutt and Lower Hutt cities by the Rimutaka Ranges. The district&apos;s northern borders are vague, and there is some overlap with southern Hawke&apos;s Bay. Part of the reason is that the area was settled from both the north and the west and has been the subject of several reorganisations of local government. The area to the north of Mt Bruce, extending through Pahiatua and Woodville to about Dannevirke, is part of the Tararua District and is in the Manawatu-Wanganui region, because it is in the catchment of the headwaters of the Manawatu River. The river runs westward between the two mountain ranges (Tararua Ranges to the south and Ruahine Ranges to the north) via the Manawatu Gorge, to pass through Palmerston North and reach the west coast of the North Island. The east coast contains settlements such as Tinui, Castlepoint, and Riversdale, while the main southern rivers drain through or past Lake Wairarapa to discharge into Palliser Bay east of Cook Strait.</obo:IAO_0000115>
        <oboInOwl:hasOBONamespace>GAZ</oboInOwl:hasOBONamespace>
        <oboInOwl:id>GAZ:00010255</oboInOwl:id>
        <rdfs:label>Wairarapa</rdfs:label>
    </owl:NamedIndividual>
    


    <!-- http://purl.obolibrary.org/obo/GAZ_00010256 -->

    <owl:NamedIndividual rdf:about="http://purl.obolibrary.org/obo/GAZ_00010256">
        <obo:RO_0001025 rdf:resource="http://purl.obolibrary.org/obo/GAZ_00004765"/>
        <obo:RO_0001025 rdf:resource="http://purl.obolibrary.org/obo/GAZ_00010255"/>
    </owl:NamedIndividual>
    


    <!-- http://purl.obolibrary.org/obo/GAZ_00010257 -->

    <owl:NamedIndividual rdf:about="http://purl.obolibrary.org/obo/GAZ_00010257">
        <obo:RO_0001025 rdf:resource="http://purl.obolibrary.org/obo/GAZ_00008567"/>
    </owl:NamedIndividual>
    


    <!-- http://purl.obolibrary.org/obo/GAZ_00010258 -->

    <owl:NamedIndividual rdf:about="http://purl.obolibrary.org/obo/GAZ_00010258">
        <obo:RO_0001025 rdf:resource="http://purl.obolibrary.org/obo/GAZ_00004772"/>
        <oboInOwl:hasOBONamespace>GAZ</oboInOwl:hasOBONamespace>
        <oboInOwl:id>GAZ:00010258</oboInOwl:id>
        <rdfs:label>Manawatu District</rdfs:label>
    </owl:NamedIndividual>
    


    <!-- http://purl.obolibrary.org/obo/GAZ_00011683 -->

    <owl:NamedIndividual rdf:about="http://purl.obolibrary.org/obo/GAZ_00011683">
        <obo:RO_0001025 rdf:resource="http://purl.obolibrary.org/obo/GAZ_00009535"/>
        <obo:IAO_0000115>The second largest lake in the North Island of New Zealand by surface area, and covers 7,878 ha. With a mean depth of only 11 m it is considerably smaller than nearby Lake Tarawera in terms of volume of water. It is located in the Bay of Plenty region. The city of Rotorua is sited on its southern shore, and the town of Ngongotaha is at the western edge of the lake. The lake was formed from the crater of a large volcano in the Taupo Volcanic Zone. Its last major eruption was about 240,000 years ago. After the eruption, the magma chamber underneath the volcano collapsed. The circular depression left behind is the Rotorua Caldera, which is the site of the lake.</obo:IAO_0000115>
        <oboInOwl:hasOBONamespace>GAZ</oboInOwl:hasOBONamespace>
        <oboInOwl:id>GAZ:00011683</oboInOwl:id>
        <rdfs:label>Lake Rotorua</rdfs:label>
    </owl:NamedIndividual>
    


    <!-- http://purl.obolibrary.org/obo/GAZ_00012588 -->

    <owl:NamedIndividual rdf:about="http://purl.obolibrary.org/obo/GAZ_00012588">
        <obo:RO_0001025 rdf:resource="http://purl.obolibrary.org/obo/GAZ_00007723"/>
        <oboInOwl:hasOBONamespace>GAZ</oboInOwl:hasOBONamespace>
        <oboInOwl:id>GAZ:00012588</oboInOwl:id>
        <rdfs:label>Whakatane District</rdfs:label>
    </owl:NamedIndividual>
    


    <!-- http://purl.obolibrary.org/obo/GAZ_00012589 -->

    <owl:NamedIndividual rdf:about="http://purl.obolibrary.org/obo/GAZ_00012589">
        <obo:RO_0001025 rdf:resource="http://purl.obolibrary.org/obo/GAZ_00004767"/>
        <obo:RO_0001025 rdf:resource="http://purl.obolibrary.org/obo/GAZ_00008562"/>
        <oboInOwl:hasOBONamespace>GAZ</oboInOwl:hasOBONamespace>
        <oboInOwl:id>GAZ:00012589</oboInOwl:id>
        <rdfs:label>Waitaki District</rdfs:label>
    </owl:NamedIndividual>
    


    <!-- http://purl.obolibrary.org/obo/GAZ_00012590 -->

    <owl:NamedIndividual rdf:about="http://purl.obolibrary.org/obo/GAZ_00012590">
        <obo:RO_0001025 rdf:resource="http://purl.obolibrary.org/obo/GAZ_00008572"/>
        <oboInOwl:hasOBONamespace>GAZ</oboInOwl:hasOBONamespace>
        <oboInOwl:id>GAZ:00012590</oboInOwl:id>
        <rdfs:label>Southland District</rdfs:label>
    </owl:NamedIndividual>
    


    <!-- http://purl.obolibrary.org/obo/GAZ_00016313 -->

    <owl:NamedIndividual rdf:about="http://purl.obolibrary.org/obo/GAZ_00016313">
        <obo:RO_0001025 rdf:resource="http://purl.obolibrary.org/obo/GAZ_00007126"/>
        <obo:IAO_0000115>An island W of Mangere Island. An eroded Pliocene volcano. The island lies off the west coast of Pitt Island, 45 km southeast of the chain&apos;s main settlement, Waitangi, on Chatham Island.</obo:IAO_0000115>
        <oboInOwl:hasOBONamespace>GAZ</oboInOwl:hasOBONamespace>
        <oboInOwl:id>GAZ:00016313</oboInOwl:id>
        <rdfs:label>Little Mangere Island</rdfs:label>
    </owl:NamedIndividual>
    


    <!-- http://purl.obolibrary.org/obo/GAZ_00016314 -->

    <owl:NamedIndividual rdf:about="http://purl.obolibrary.org/obo/GAZ_00016314">
        <obo:RO_0001025 rdf:resource="http://purl.obolibrary.org/obo/GAZ_00016319"/>
        <oboInOwl:hasOBONamespace>GAZ</oboInOwl:hasOBONamespace>
        <oboInOwl:id>GAZ:00016314</oboInOwl:id>
        <rdfs:label>Round Islet</rdfs:label>
    </owl:NamedIndividual>
    


    <!-- http://purl.obolibrary.org/obo/GAZ_00016315 -->

    <owl:NamedIndividual rdf:about="http://purl.obolibrary.org/obo/GAZ_00016315">
        <obo:RO_0001025 rdf:resource="http://purl.obolibrary.org/obo/GAZ_00007126"/>
        <obo:IAO_0000115>A part of the Chatham Islands group, located 800 km east of New Zealand&apos;s South Island. The islands lie 50 km east of the group&apos;s main island, Chatham Island.</obo:IAO_0000115>
        <oboInOwl:hasOBONamespace>GAZ</oboInOwl:hasOBONamespace>
        <oboInOwl:id>GAZ:00016315</oboInOwl:id>
        <rdfs:label>Forty-Fours Islands</rdfs:label>
    </owl:NamedIndividual>
    


    <!-- http://purl.obolibrary.org/obo/GAZ_00016316 -->

    <owl:NamedIndividual rdf:about="http://purl.obolibrary.org/obo/GAZ_00016316">
        <obo:RO_0001025 rdf:resource="http://purl.obolibrary.org/obo/GAZ_00007126"/>
        <obo:IAO_0000115>The second largest island in the Chatham Islands.</obo:IAO_0000115>
        <oboInOwl:hasOBONamespace>GAZ</oboInOwl:hasOBONamespace>
        <oboInOwl:id>GAZ:00016316</oboInOwl:id>
        <rdfs:label>Pitt Island</rdfs:label>
    </owl:NamedIndividual>
    


    <!-- http://purl.obolibrary.org/obo/GAZ_00016317 -->

    <owl:NamedIndividual rdf:about="http://purl.obolibrary.org/obo/GAZ_00016317">
        <obo:RO_0001025 rdf:resource="http://purl.obolibrary.org/obo/GAZ_00007126"/>
        <obo:IAO_0000115>An island to the W of Pitt Island. An eroded Pliocene volcano.</obo:IAO_0000115>
        <oboInOwl:hasOBONamespace>GAZ</oboInOwl:hasOBONamespace>
        <oboInOwl:id>GAZ:00016317</oboInOwl:id>
        <rdfs:label>Mangere Island</rdfs:label>
    </owl:NamedIndividual>
    


    <!-- http://purl.obolibrary.org/obo/GAZ_00016318 -->

    <owl:NamedIndividual rdf:about="http://purl.obolibrary.org/obo/GAZ_00016318">
        <obo:RO_0001025 rdf:resource="http://purl.obolibrary.org/obo/GAZ_00007126"/>
        <obo:IAO_0000115>The largest island of the Chatham Islands group, in the south Pacific Ocean off the eastern coast of New Zealand.</obo:IAO_0000115>
        <oboInOwl:hasOBONamespace>GAZ</oboInOwl:hasOBONamespace>
        <oboInOwl:id>GAZ:00016318</oboInOwl:id>
        <rdfs:label>Chatham Island</rdfs:label>
    </owl:NamedIndividual>
    


    <!-- http://purl.obolibrary.org/obo/GAZ_00016319 -->

    <owl:NamedIndividual rdf:about="http://purl.obolibrary.org/obo/GAZ_00016319">
        <obo:RO_0001025 rdf:resource="http://purl.obolibrary.org/obo/GAZ_00007126"/>
        <obo:IAO_0000115>A part of the Chatham Islands chain, located 800 km east of New Zealand&apos;s South Island. It is a group of five rocky islets (of which Round Islet is the largest), located 12 km east of Pitt Island.</obo:IAO_0000115>
        <oboInOwl:hasOBONamespace>GAZ</oboInOwl:hasOBONamespace>
        <oboInOwl:id>GAZ:00016319</oboInOwl:id>
        <rdfs:label>Star Keys</rdfs:label>
    </owl:NamedIndividual>
    


    <!-- http://purl.obolibrary.org/obo/GAZ_00016320 -->

    <owl:NamedIndividual rdf:about="http://purl.obolibrary.org/obo/GAZ_00016320">
        <obo:RO_0001025 rdf:resource="http://purl.obolibrary.org/obo/GAZ_00007126"/>
        <obo:IAO_0000115>Part of the Chatham Islands chain, located 800 km east of New Zealand&apos;s South Island. The northernmost part of the group, they lie 16 km north of Cape Pattison on Chatham Island. Consists of 5 or 6 small islands.</obo:IAO_0000115>
        <oboInOwl:hasOBONamespace>GAZ</oboInOwl:hasOBONamespace>
        <oboInOwl:id>GAZ:00016320</oboInOwl:id>
        <rdfs:label>The Sisters</rdfs:label>
    </owl:NamedIndividual>
    


    <!-- http://purl.obolibrary.org/obo/GAZ_00016321 -->

    <owl:NamedIndividual rdf:about="http://purl.obolibrary.org/obo/GAZ_00016321">
        <obo:RO_0001025 rdf:resource="http://purl.obolibrary.org/obo/GAZ_00007126"/>
        <obo:IAO_0000115>An island SE of Pitt Island. It off the southeast coast of Pitt Island, 55 km southeast of the chain&apos;s main settlement, Waitangi, on Chatham Island.</obo:IAO_0000115>
        <oboInOwl:hasOBONamespace>GAZ</oboInOwl:hasOBONamespace>
        <oboInOwl:id>GAZ:00016321</oboInOwl:id>
        <rdfs:label>South East Island</rdfs:label>
    </owl:NamedIndividual>
    


    <!-- http://purl.obolibrary.org/obo/GAZ_00016679 -->

    <owl:NamedIndividual rdf:about="http://purl.obolibrary.org/obo/GAZ_00016679">
        <obo:RO_0001025 rdf:resource="http://purl.obolibrary.org/obo/GAZ_00046925"/>
        <obo:IAO_0000115>An island in the Marlborough Sounds along the northern coast of the South Island of New Zealand.</obo:IAO_0000115>
        <oboInOwl:hasOBONamespace>GAZ</oboInOwl:hasOBONamespace>
        <oboInOwl:id>GAZ:00016679</oboInOwl:id>
        <rdfs:label>D&apos;Urville Island</rdfs:label>
    </owl:NamedIndividual>
    


    <!-- http://purl.obolibrary.org/obo/GAZ_00016680 -->

    <owl:NamedIndividual rdf:about="http://purl.obolibrary.org/obo/GAZ_00016680">
        <obo:RO_0001025 rdf:resource="http://purl.obolibrary.org/obo/GAZ_00046945"/>
        <oboInOwl:hasOBONamespace>GAZ</oboInOwl:hasOBONamespace>
        <oboInOwl:id>GAZ:00016680</oboInOwl:id>
        <rdfs:label>Great Barrier Island</rdfs:label>
    </owl:NamedIndividual>
    


    <!-- http://purl.obolibrary.org/obo/GAZ_00016691 -->

    <owl:NamedIndividual rdf:about="http://purl.obolibrary.org/obo/GAZ_00016691">
        <obo:RO_0001025 rdf:resource="http://purl.obolibrary.org/obo/GAZ_00046945"/>
        <obo:IAO_0000115>An island in the Hauraki Gulf of New Zealand and is located about 17.7 km from Auckland.</obo:IAO_0000115>
        <oboInOwl:hasOBONamespace>GAZ</oboInOwl:hasOBONamespace>
        <oboInOwl:id>GAZ:00016691</oboInOwl:id>
        <rdfs:label>Waiheke Island</rdfs:label>
    </owl:NamedIndividual>
    


    <!-- http://purl.obolibrary.org/obo/GAZ_00016975 -->

    <owl:NamedIndividual rdf:about="http://purl.obolibrary.org/obo/GAZ_00016975">
        <obo:RO_0001025 rdf:resource="http://purl.obolibrary.org/obo/GAZ_00142025"/>
        <obo:IAO_0000115>The major and NW of the Atafu Islands.</obo:IAO_0000115>
        <oboInOwl:hasOBONamespace>GAZ</oboInOwl:hasOBONamespace>
        <oboInOwl:id>GAZ:00016975</oboInOwl:id>
        <rdfs:label>Atafu Island</rdfs:label>
    </owl:NamedIndividual>
    


    <!-- http://purl.obolibrary.org/obo/GAZ_00016977 -->

    <owl:NamedIndividual rdf:about="http://purl.obolibrary.org/obo/GAZ_00016977">
        <obo:RO_0001025 rdf:resource="http://purl.obolibrary.org/obo/GAZ_00009561"/>
        <obo:IAO_0000115>An island of the Fakaofo Atoll.</obo:IAO_0000115>
        <oboInOwl:hasOBONamespace>GAZ</oboInOwl:hasOBONamespace>
        <oboInOwl:id>GAZ:00016977</oboInOwl:id>
        <rdfs:label>Teafua</rdfs:label>
    </owl:NamedIndividual>
    


    <!-- http://purl.obolibrary.org/obo/GAZ_00016978 -->

    <owl:NamedIndividual rdf:about="http://purl.obolibrary.org/obo/GAZ_00016978">
        <obo:RO_0001025 rdf:resource="http://purl.obolibrary.org/obo/GAZ_00142131"/>
        <obo:IAO_0000115>An island on the NE rim of the Fakaofo Atoll.</obo:IAO_0000115>
        <oboInOwl:hasOBONamespace>GAZ</oboInOwl:hasOBONamespace>
        <oboInOwl:id>GAZ:00016978</oboInOwl:id>
        <rdfs:label>Mulifenua</rdfs:label>
    </owl:NamedIndividual>
    


    <!-- http://purl.obolibrary.org/obo/GAZ_00016979 -->

    <owl:NamedIndividual rdf:about="http://purl.obolibrary.org/obo/GAZ_00016979">
        <obo:RO_0001025 rdf:resource="http://purl.obolibrary.org/obo/GAZ_00142136"/>
        <obo:IAO_0000115>The main island of the Fakaofo Atoll, on the S.</obo:IAO_0000115>
        <oboInOwl:hasOBONamespace>GAZ</oboInOwl:hasOBONamespace>
        <oboInOwl:id>GAZ:00016979</oboInOwl:id>
        <rdfs:label>Fenua Loa</rdfs:label>
    </owl:NamedIndividual>
    


    <!-- http://purl.obolibrary.org/obo/GAZ_00016980 -->

    <owl:NamedIndividual rdf:about="http://purl.obolibrary.org/obo/GAZ_00016980">
        <obo:RO_0001025 rdf:resource="http://purl.obolibrary.org/obo/GAZ_00009561"/>
        <obo:IAO_0000115>An island of the Fakaofo Atoll.</obo:IAO_0000115>
        <oboInOwl:hasOBONamespace>GAZ</oboInOwl:hasOBONamespace>
        <oboInOwl:id>GAZ:00016980</oboInOwl:id>
        <rdfs:label>Lalo</rdfs:label>
    </owl:NamedIndividual>
    


    <!-- http://purl.obolibrary.org/obo/GAZ_00016981 -->

    <owl:NamedIndividual rdf:about="http://purl.obolibrary.org/obo/GAZ_00016981">
        <obo:RO_0001025 rdf:resource="http://purl.obolibrary.org/obo/GAZ_00142132"/>
        <obo:IAO_0000115>An island on the E rim of the Fakaofo Atoll.</obo:IAO_0000115>
        <oboInOwl:hasOBONamespace>GAZ</oboInOwl:hasOBONamespace>
        <oboInOwl:id>GAZ:00016981</oboInOwl:id>
        <rdfs:label>Motu Akea</rdfs:label>
    </owl:NamedIndividual>
    


    <!-- http://purl.obolibrary.org/obo/GAZ_00016982 -->

    <owl:NamedIndividual rdf:about="http://purl.obolibrary.org/obo/GAZ_00016982">
        <obo:RO_0001025 rdf:resource="http://purl.obolibrary.org/obo/GAZ_00142137"/>
        <obo:IAO_0000115>An island on the SW rim of the Fakaofo Atoll.</obo:IAO_0000115>
        <oboInOwl:hasOBONamespace>GAZ</oboInOwl:hasOBONamespace>
        <oboInOwl:id>GAZ:00016982</oboInOwl:id>
        <rdfs:label>Nukulakia</rdfs:label>
    </owl:NamedIndividual>
    


    <!-- http://purl.obolibrary.org/obo/GAZ_00016983 -->

    <owl:NamedIndividual rdf:about="http://purl.obolibrary.org/obo/GAZ_00016983">
        <obo:RO_0001025 rdf:resource="http://purl.obolibrary.org/obo/GAZ_00009561"/>
        <obo:IAO_0000115>An island of the Fakaofo Atoll.</obo:IAO_0000115>
        <oboInOwl:hasOBONamespace>GAZ</oboInOwl:hasOBONamespace>
        <oboInOwl:id>GAZ:00016983</oboInOwl:id>
        <rdfs:label>Saumatafanga</rdfs:label>
    </owl:NamedIndividual>
    


    <!-- http://purl.obolibrary.org/obo/GAZ_00016984 -->

    <owl:NamedIndividual rdf:about="http://purl.obolibrary.org/obo/GAZ_00016984">
        <obo:RO_0001025 rdf:resource="http://purl.obolibrary.org/obo/GAZ_00009561"/>
        <obo:IAO_0000115>An island of the Fakaofo Atoll.</obo:IAO_0000115>
        <oboInOwl:hasOBONamespace>GAZ</oboInOwl:hasOBONamespace>
        <oboInOwl:id>GAZ:00016984</oboInOwl:id>
        <rdfs:label>Matangi</rdfs:label>
    </owl:NamedIndividual>
    


    <!-- http://purl.obolibrary.org/obo/GAZ_00016985 -->

    <owl:NamedIndividual rdf:about="http://purl.obolibrary.org/obo/GAZ_00016985">
        <obo:RO_0001025 rdf:resource="http://purl.obolibrary.org/obo/GAZ_00142137"/>
        <obo:IAO_0000115>An island on the SW rim of the Fakaofo Atoll.</obo:IAO_0000115>
        <oboInOwl:hasOBONamespace>GAZ</oboInOwl:hasOBONamespace>
        <oboInOwl:id>GAZ:00016985</oboInOwl:id>
        <rdfs:label>Nukumatau</rdfs:label>
    </owl:NamedIndividual>
    


    <!-- http://purl.obolibrary.org/obo/GAZ_00016987 -->

    <owl:NamedIndividual rdf:about="http://purl.obolibrary.org/obo/GAZ_00016987">
        <obo:RO_0001025 rdf:resource="http://purl.obolibrary.org/obo/GAZ_00142066"/>
        <obo:IAO_0000115>An island on the W rim of the Atafu Atoll.</obo:IAO_0000115>
        <oboInOwl:hasOBONamespace>GAZ</oboInOwl:hasOBONamespace>
        <oboInOwl:id>GAZ:00016987</oboInOwl:id>
        <rdfs:label>Kauafua</rdfs:label>
    </owl:NamedIndividual>
    


    <!-- http://purl.obolibrary.org/obo/GAZ_00016988 -->

    <owl:NamedIndividual rdf:about="http://purl.obolibrary.org/obo/GAZ_00016988">
        <obo:RO_0001025 rdf:resource="http://purl.obolibrary.org/obo/GAZ_00009562"/>
        <oboInOwl:hasOBONamespace>GAZ</oboInOwl:hasOBONamespace>
        <oboInOwl:id>GAZ:00016988</oboInOwl:id>
        <rdfs:label>Tamaseko Island</rdfs:label>
    </owl:NamedIndividual>
    


    <!-- http://purl.obolibrary.org/obo/GAZ_00016989 -->

    <owl:NamedIndividual rdf:about="http://purl.obolibrary.org/obo/GAZ_00016989">
        <obo:RO_0001025 rdf:resource="http://purl.obolibrary.org/obo/GAZ_00142120"/>
        <obo:IAO_0000115>An island in the Nukunonu Atoll, on the SW rim.</obo:IAO_0000115>
        <oboInOwl:hasOBONamespace>GAZ</oboInOwl:hasOBONamespace>
        <oboInOwl:id>GAZ:00016989</oboInOwl:id>
        <rdfs:label>Nukunonu</rdfs:label>
    </owl:NamedIndividual>
    


    <!-- http://purl.obolibrary.org/obo/GAZ_00016991 -->

    <owl:NamedIndividual rdf:about="http://purl.obolibrary.org/obo/GAZ_00016991">
        <obo:RO_0001025 rdf:resource="http://purl.obolibrary.org/obo/GAZ_00142120"/>
        <obo:IAO_0000115>An island in the Nukunonu Atoll.</obo:IAO_0000115>
        <oboInOwl:hasOBONamespace>GAZ</oboInOwl:hasOBONamespace>
        <oboInOwl:id>GAZ:00016991</oboInOwl:id>
        <rdfs:label>Motuhaga</rdfs:label>
    </owl:NamedIndividual>
    


    <!-- http://purl.obolibrary.org/obo/GAZ_00016992 -->

    <owl:NamedIndividual rdf:about="http://purl.obolibrary.org/obo/GAZ_00016992">
        <obo:RO_0001025 rdf:resource="http://purl.obolibrary.org/obo/GAZ_00009560"/>
        <obo:IAO_0000115>An island in the Nukunonu Atoll, on the NW rim.</obo:IAO_0000115>
        <oboInOwl:hasOBONamespace>GAZ</oboInOwl:hasOBONamespace>
        <oboInOwl:id>GAZ:00016992</oboInOwl:id>
        <rdfs:label>Te Fakanava</rdfs:label>
    </owl:NamedIndividual>
    


    <!-- http://purl.obolibrary.org/obo/GAZ_00016993 -->

    <owl:NamedIndividual rdf:about="http://purl.obolibrary.org/obo/GAZ_00016993">
        <obo:RO_0001025 rdf:resource="http://purl.obolibrary.org/obo/GAZ_00142113"/>
        <obo:IAO_0000115>An island in the Nukunonu Atoll.</obo:IAO_0000115>
        <oboInOwl:hasOBONamespace>GAZ</oboInOwl:hasOBONamespace>
        <oboInOwl:id>GAZ:00016993</oboInOwl:id>
        <rdfs:label>Avakilikili</rdfs:label>
    </owl:NamedIndividual>
    


    <!-- http://purl.obolibrary.org/obo/GAZ_00016994 -->

    <owl:NamedIndividual rdf:about="http://purl.obolibrary.org/obo/GAZ_00016994">
        <obo:RO_0001025 rdf:resource="http://purl.obolibrary.org/obo/GAZ_00009560"/>
        <obo:IAO_0000115>An island in the Nukunonu Atoll.</obo:IAO_0000115>
        <oboInOwl:hasOBONamespace>GAZ</oboInOwl:hasOBONamespace>
        <oboInOwl:id>GAZ:00016994</oboInOwl:id>
        <rdfs:label>Te Puku</rdfs:label>
    </owl:NamedIndividual>
    


    <!-- http://purl.obolibrary.org/obo/GAZ_00016995 -->

    <owl:NamedIndividual rdf:about="http://purl.obolibrary.org/obo/GAZ_00016995">
        <obo:RO_0001025 rdf:resource="http://purl.obolibrary.org/obo/GAZ_00009560"/>
        <obo:IAO_0000115>An island in the Nukunonu Atoll.</obo:IAO_0000115>
        <oboInOwl:hasOBONamespace>GAZ</oboInOwl:hasOBONamespace>
        <oboInOwl:id>GAZ:00016995</oboInOwl:id>
        <rdfs:label>Laulauia</rdfs:label>
    </owl:NamedIndividual>
    


    <!-- http://purl.obolibrary.org/obo/GAZ_00016996 -->

    <owl:NamedIndividual rdf:about="http://purl.obolibrary.org/obo/GAZ_00016996">
        <obo:RO_0001025 rdf:resource="http://purl.obolibrary.org/obo/GAZ_00142120"/>
        <obo:IAO_0000115>An island in the Nukunonu Atoll, on the S rim.</obo:IAO_0000115>
        <oboInOwl:hasOBONamespace>GAZ</oboInOwl:hasOBONamespace>
        <oboInOwl:id>GAZ:00016996</oboInOwl:id>
        <rdfs:label>Fatigauhu</rdfs:label>
    </owl:NamedIndividual>
    


    <!-- http://purl.obolibrary.org/obo/GAZ_00016997 -->

    <owl:NamedIndividual rdf:about="http://purl.obolibrary.org/obo/GAZ_00016997">
        <obo:RO_0001025 rdf:resource="http://purl.obolibrary.org/obo/GAZ_00142117"/>
        <obo:IAO_0000115>An island in the Nukunonu Atoll.</obo:IAO_0000115>
        <oboInOwl:hasOBONamespace>GAZ</oboInOwl:hasOBONamespace>
        <oboInOwl:id>GAZ:00016997</oboInOwl:id>
        <rdfs:label>Te Kamu</rdfs:label>
    </owl:NamedIndividual>
    


    <!-- http://purl.obolibrary.org/obo/GAZ_00016998 -->

    <owl:NamedIndividual rdf:about="http://purl.obolibrary.org/obo/GAZ_00016998">
        <obo:RO_0001025 rdf:resource="http://purl.obolibrary.org/obo/GAZ_00009560"/>
        <obo:IAO_0000115>An island in the Nukunonu Atoll.</obo:IAO_0000115>
        <oboInOwl:hasOBONamespace>GAZ</oboInOwl:hasOBONamespace>
        <oboInOwl:id>GAZ:00016998</oboInOwl:id>
        <rdfs:label>Saumagalu</rdfs:label>
    </owl:NamedIndividual>
    


    <!-- http://purl.obolibrary.org/obo/GAZ_00016999 -->

    <owl:NamedIndividual rdf:about="http://purl.obolibrary.org/obo/GAZ_00016999">
        <obo:RO_0001025 rdf:resource="http://purl.obolibrary.org/obo/GAZ_00009560"/>
        <obo:IAO_0000115>An island in the Nukunonu Atoll.</obo:IAO_0000115>
        <oboInOwl:hasOBONamespace>GAZ</oboInOwl:hasOBONamespace>
        <oboInOwl:id>GAZ:00016999</oboInOwl:id>
        <rdfs:label>Taulagapapa</rdfs:label>
    </owl:NamedIndividual>
    


    <!-- http://purl.obolibrary.org/obo/GAZ_00017000 -->

    <owl:NamedIndividual rdf:about="http://purl.obolibrary.org/obo/GAZ_00017000">
        <obo:RO_0001025 rdf:resource="http://purl.obolibrary.org/obo/GAZ_00142121"/>
        <obo:IAO_0000115>An island in the Nukunonu Atoll.</obo:IAO_0000115>
        <oboInOwl:hasOBONamespace>GAZ</oboInOwl:hasOBONamespace>
        <oboInOwl:id>GAZ:00017000</oboInOwl:id>
        <rdfs:label>Punalei</rdfs:label>
    </owl:NamedIndividual>
    


    <!-- http://purl.obolibrary.org/obo/GAZ_00017001 -->

    <owl:NamedIndividual rdf:about="http://purl.obolibrary.org/obo/GAZ_00017001">
        <obo:RO_0001025 rdf:resource="http://purl.obolibrary.org/obo/GAZ_00142113"/>
        <obo:IAO_0000115>An island in the Nukunonu Atoll.</obo:IAO_0000115>
        <oboInOwl:hasOBONamespace>GAZ</oboInOwl:hasOBONamespace>
        <oboInOwl:id>GAZ:00017001</oboInOwl:id>
        <rdfs:label>Apia</rdfs:label>
    </owl:NamedIndividual>
    


    <!-- http://purl.obolibrary.org/obo/GAZ_00017002 -->

    <owl:NamedIndividual rdf:about="http://purl.obolibrary.org/obo/GAZ_00017002">
        <obo:RO_0001025 rdf:resource="http://purl.obolibrary.org/obo/GAZ_00142113"/>
        <obo:IAO_0000115>An island in the Nukunonu Atoll.</obo:IAO_0000115>
        <oboInOwl:hasOBONamespace>GAZ</oboInOwl:hasOBONamespace>
        <oboInOwl:id>GAZ:00017002</oboInOwl:id>
        <rdfs:label>Niututahi</rdfs:label>
    </owl:NamedIndividual>
    


    <!-- http://purl.obolibrary.org/obo/GAZ_00017003 -->

    <owl:NamedIndividual rdf:about="http://purl.obolibrary.org/obo/GAZ_00017003">
        <obo:RO_0001025 rdf:resource="http://purl.obolibrary.org/obo/GAZ_00009560"/>
        <obo:IAO_0000115>An island in the Nukunonu Atoll.</obo:IAO_0000115>
        <oboInOwl:hasOBONamespace>GAZ</oboInOwl:hasOBONamespace>
        <oboInOwl:id>GAZ:00017003</oboInOwl:id>
        <rdfs:label>Ahua</rdfs:label>
    </owl:NamedIndividual>
    


    <!-- http://purl.obolibrary.org/obo/GAZ_00017004 -->

    <owl:NamedIndividual rdf:about="http://purl.obolibrary.org/obo/GAZ_00017004">
        <obo:RO_0001025 rdf:resource="http://purl.obolibrary.org/obo/GAZ_00142120"/>
        <obo:IAO_0000115>An island in the Nukunonu Atoll, on the SW rim.</obo:IAO_0000115>
        <oboInOwl:hasOBONamespace>GAZ</oboInOwl:hasOBONamespace>
        <oboInOwl:id>GAZ:00017004</oboInOwl:id>
        <rdfs:label>Te Puka e Mua</rdfs:label>
    </owl:NamedIndividual>
    


    <!-- http://purl.obolibrary.org/obo/GAZ_00017005 -->

    <owl:NamedIndividual rdf:about="http://purl.obolibrary.org/obo/GAZ_00017005">
        <obo:RO_0001025 rdf:resource="http://purl.obolibrary.org/obo/GAZ_00142121"/>
        <obo:IAO_0000115>An island in the Nukunonu Atoll.</obo:IAO_0000115>
        <oboInOwl:hasOBONamespace>GAZ</oboInOwl:hasOBONamespace>
        <oboInOwl:id>GAZ:00017005</oboInOwl:id>
        <rdfs:label>Motufala</rdfs:label>
    </owl:NamedIndividual>
    


    <!-- http://purl.obolibrary.org/obo/GAZ_00017414 -->

    <owl:NamedIndividual rdf:about="http://purl.obolibrary.org/obo/GAZ_00017414">
        <obo:RO_0001025 rdf:resource="http://purl.obolibrary.org/obo/GAZ_00007173"/>
        <obo:IAO_0000115>An uninhabited island, part of the Auckland Islands group, a subantarctic chain that forms part of the New Zealand Outlying Islands. Ewing Island is located in the northeast of the group, close to the mouth of Port Ross, immediately to the south of the larger Enderby Island and off the northeastern tip of the main Auckland Island.</obo:IAO_0000115>
        <oboInOwl:hasOBONamespace>GAZ</oboInOwl:hasOBONamespace>
        <oboInOwl:id>GAZ:00017414</oboInOwl:id>
        <rdfs:label>Ewing Island</rdfs:label>
    </owl:NamedIndividual>
    


    <!-- http://purl.obolibrary.org/obo/GAZ_00017415 -->

    <owl:NamedIndividual rdf:about="http://purl.obolibrary.org/obo/GAZ_00017415">
        <obo:RO_0001025 rdf:resource="http://purl.obolibrary.org/obo/GAZ_00007173"/>
        <obo:IAO_0000115>One of the Auckland Islands, to the E of Auckland Island.</obo:IAO_0000115>
        <oboInOwl:hasOBONamespace>GAZ</oboInOwl:hasOBONamespace>
        <oboInOwl:id>GAZ:00017415</oboInOwl:id>
        <rdfs:label>Dundas Island</rdfs:label>
    </owl:NamedIndividual>
    


    <!-- http://purl.obolibrary.org/obo/GAZ_00017416 -->

    <owl:NamedIndividual rdf:about="http://purl.obolibrary.org/obo/GAZ_00017416">
        <obo:RO_0001025 rdf:resource="http://purl.obolibrary.org/obo/GAZ_00007173"/>
        <obo:IAO_0000115>One of the Auckland Islands, to the E of Auckland Island.</obo:IAO_0000115>
        <oboInOwl:hasOBONamespace>GAZ</oboInOwl:hasOBONamespace>
        <oboInOwl:id>GAZ:00017416</oboInOwl:id>
        <rdfs:label>Green Island</rdfs:label>
    </owl:NamedIndividual>
    


    <!-- http://purl.obolibrary.org/obo/GAZ_00017417 -->

    <owl:NamedIndividual rdf:about="http://purl.obolibrary.org/obo/GAZ_00017417">
        <obo:RO_0001025 rdf:resource="http://purl.obolibrary.org/obo/GAZ_00007173"/>
        <obo:IAO_0000115>An island of the Auckland Islands archipelago. The southern end of Auckland Island broadens to a width of 26 km where a narrow channel, known as Carnley Harbour or the Adams Straits, separates it from the roughly triangular Adams Island (area approximately 100 km2), which is even more mountainous, reaching a height of 705 m at Mount Dick.</obo:IAO_0000115>
        <oboInOwl:hasOBONamespace>GAZ</oboInOwl:hasOBONamespace>
        <oboInOwl:id>GAZ:00017417</oboInOwl:id>
        <rdfs:label>Adams Island</rdfs:label>
    </owl:NamedIndividual>
    


    <!-- http://purl.obolibrary.org/obo/GAZ_00017418 -->

    <owl:NamedIndividual rdf:about="http://purl.obolibrary.org/obo/GAZ_00017418">
        <obo:RO_0001025 rdf:resource="http://purl.obolibrary.org/obo/GAZ_00007173"/>
        <obo:IAO_0000115>The main island of the Auckland Islands, an uninhabited archipelago in the south Pacific Ocean belonging to New Zealand.</obo:IAO_0000115>
        <oboInOwl:hasOBONamespace>GAZ</oboInOwl:hasOBONamespace>
        <oboInOwl:id>GAZ:00017418</oboInOwl:id>
        <rdfs:label>Auckland Island</rdfs:label>
    </owl:NamedIndividual>
    


    <!-- http://purl.obolibrary.org/obo/GAZ_00017419 -->

    <owl:NamedIndividual rdf:about="http://purl.obolibrary.org/obo/GAZ_00017419">
        <obo:RO_0001025 rdf:resource="http://purl.obolibrary.org/obo/GAZ_00007173"/>
        <obo:IAO_0000115>An island in the Aukland Islands. It is five miles from the north-west end of Auckland Island and 180 miles south of New Zealand.</obo:IAO_0000115>
        <oboInOwl:hasOBONamespace>GAZ</oboInOwl:hasOBONamespace>
        <oboInOwl:id>GAZ:00017419</oboInOwl:id>
        <rdfs:label>Disappointment Island</rdfs:label>
    </owl:NamedIndividual>
    


    <!-- http://purl.obolibrary.org/obo/GAZ_00017420 -->

    <owl:NamedIndividual rdf:about="http://purl.obolibrary.org/obo/GAZ_00017420">
        <obo:RO_0001025 rdf:resource="http://purl.obolibrary.org/obo/GAZ_00007173"/>
        <obo:IAO_0000115>An island of the Auckland Islands archipelago. It is situated just off the northern tip of Auckland Island, the largest island in the archipelago.</obo:IAO_0000115>
        <oboInOwl:hasOBONamespace>GAZ</oboInOwl:hasOBONamespace>
        <oboInOwl:id>GAZ:00017420</oboInOwl:id>
        <rdfs:label>Enderby Island</rdfs:label>
    </owl:NamedIndividual>
    


    <!-- http://purl.obolibrary.org/obo/GAZ_00017421 -->

    <owl:NamedIndividual rdf:about="http://purl.obolibrary.org/obo/GAZ_00017421">
        <obo:RO_0001025 rdf:resource="http://purl.obolibrary.org/obo/GAZ_00007172"/>
        <obo:IAO_0000115>A small island of the Antipodes Islands Group.</obo:IAO_0000115>
        <oboInOwl:hasOBONamespace>GAZ</oboInOwl:hasOBONamespace>
        <oboInOwl:id>GAZ:00017421</oboInOwl:id>
        <rdfs:label>Bollons Island</rdfs:label>
    </owl:NamedIndividual>
    


    <!-- http://purl.obolibrary.org/obo/GAZ_00017422 -->

    <owl:NamedIndividual rdf:about="http://purl.obolibrary.org/obo/GAZ_00017422">
        <obo:RO_0001025 rdf:resource="http://purl.obolibrary.org/obo/GAZ_00007174"/>
        <oboInOwl:hasOBONamespace>GAZ</oboInOwl:hasOBONamespace>
        <oboInOwl:id>GAZ:00017422</oboInOwl:id>
        <rdfs:label>Centre Group</rdfs:label>
    </owl:NamedIndividual>
    


    <!-- http://purl.obolibrary.org/obo/GAZ_00017423 -->

    <owl:NamedIndividual rdf:about="http://purl.obolibrary.org/obo/GAZ_00017423">
        <obo:RO_0001025 rdf:resource="http://purl.obolibrary.org/obo/GAZ_00007174"/>
        <oboInOwl:hasOBONamespace>GAZ</oboInOwl:hasOBONamespace>
        <oboInOwl:id>GAZ:00017423</oboInOwl:id>
        <rdfs:label>East Group</rdfs:label>
    </owl:NamedIndividual>
    


    <!-- http://purl.obolibrary.org/obo/GAZ_00017424 -->

    <owl:NamedIndividual rdf:about="http://purl.obolibrary.org/obo/GAZ_00017424">
        <obo:RO_0001025 rdf:resource="http://purl.obolibrary.org/obo/GAZ_00007174"/>
        <oboInOwl:hasOBONamespace>GAZ</oboInOwl:hasOBONamespace>
        <oboInOwl:id>GAZ:00017424</oboInOwl:id>
        <rdfs:label>Main Group</rdfs:label>
    </owl:NamedIndividual>
    


    <!-- http://purl.obolibrary.org/obo/GAZ_00017425 -->

    <owl:NamedIndividual rdf:about="http://purl.obolibrary.org/obo/GAZ_00017425">
        <obo:RO_0001025 rdf:resource="http://purl.obolibrary.org/obo/GAZ_00017424"/>
        <obo:IAO_0000115>An island in the Main Group of the Bounty Islands.</obo:IAO_0000115>
        <oboInOwl:hasOBONamespace>GAZ</oboInOwl:hasOBONamespace>
        <oboInOwl:id>GAZ:00017425</oboInOwl:id>
        <rdfs:label>Lion Island</rdfs:label>
    </owl:NamedIndividual>
    


    <!-- http://purl.obolibrary.org/obo/GAZ_00017426 -->

    <owl:NamedIndividual rdf:about="http://purl.obolibrary.org/obo/GAZ_00017426">
        <obo:RO_0001025 rdf:resource="http://purl.obolibrary.org/obo/GAZ_00017424"/>
        <obo:IAO_0000115>An island in the Main Group of the Bounty Islands.</obo:IAO_0000115>
        <oboInOwl:hasOBONamespace>GAZ</oboInOwl:hasOBONamespace>
        <oboInOwl:id>GAZ:00017426</oboInOwl:id>
        <rdfs:label>Tunnel Island</rdfs:label>
    </owl:NamedIndividual>
    


    <!-- http://purl.obolibrary.org/obo/GAZ_00017427 -->

    <owl:NamedIndividual rdf:about="http://purl.obolibrary.org/obo/GAZ_00017427">
        <obo:RO_0001025 rdf:resource="http://purl.obolibrary.org/obo/GAZ_00017424"/>
        <obo:IAO_0000115>An island in the Main Group of the Bounty Islands.</obo:IAO_0000115>
        <oboInOwl:hasOBONamespace>GAZ</oboInOwl:hasOBONamespace>
        <oboInOwl:id>GAZ:00017427</oboInOwl:id>
        <rdfs:label>Spider Island</rdfs:label>
    </owl:NamedIndividual>
    


    <!-- http://purl.obolibrary.org/obo/GAZ_00017428 -->

    <owl:NamedIndividual rdf:about="http://purl.obolibrary.org/obo/GAZ_00017428">
        <obo:RO_0001025 rdf:resource="http://purl.obolibrary.org/obo/GAZ_00017424"/>
        <obo:IAO_0000115>An island in the Main Group of the Bounty Islands.</obo:IAO_0000115>
        <oboInOwl:hasOBONamespace>GAZ</oboInOwl:hasOBONamespace>
        <oboInOwl:id>GAZ:00017428</oboInOwl:id>
        <rdfs:label>Ranfurly Island</rdfs:label>
    </owl:NamedIndividual>
    


    <!-- http://purl.obolibrary.org/obo/GAZ_00017429 -->

    <owl:NamedIndividual rdf:about="http://purl.obolibrary.org/obo/GAZ_00017429">
        <obo:RO_0001025 rdf:resource="http://purl.obolibrary.org/obo/GAZ_00017424"/>
        <obo:IAO_0000115>An island in the Main Group of the Bounty Islands.</obo:IAO_0000115>
        <oboInOwl:hasOBONamespace>GAZ</oboInOwl:hasOBONamespace>
        <oboInOwl:id>GAZ:00017429</oboInOwl:id>
        <rdfs:label>Proclamation Island</rdfs:label>
    </owl:NamedIndividual>
    


    <!-- http://purl.obolibrary.org/obo/GAZ_00017430 -->

    <owl:NamedIndividual rdf:about="http://purl.obolibrary.org/obo/GAZ_00017430">
        <obo:RO_0001025 rdf:resource="http://purl.obolibrary.org/obo/GAZ_00017424"/>
        <obo:IAO_0000115>An island in the Main Group of the Bounty Islands.</obo:IAO_0000115>
        <oboInOwl:hasOBONamespace>GAZ</oboInOwl:hasOBONamespace>
        <oboInOwl:id>GAZ:00017430</oboInOwl:id>
        <rdfs:label>Depot Island</rdfs:label>
    </owl:NamedIndividual>
    


    <!-- http://purl.obolibrary.org/obo/GAZ_00017431 -->

    <owl:NamedIndividual rdf:about="http://purl.obolibrary.org/obo/GAZ_00017431">
        <obo:RO_0001025 rdf:resource="http://purl.obolibrary.org/obo/GAZ_00017422"/>
        <obo:IAO_0000115>An island in the Centre Group of the Bounty Islands.</obo:IAO_0000115>
        <oboInOwl:hasOBONamespace>GAZ</oboInOwl:hasOBONamespace>
        <oboInOwl:id>GAZ:00017431</oboInOwl:id>
        <rdfs:label>Prion Island</rdfs:label>
    </owl:NamedIndividual>
    


    <!-- http://purl.obolibrary.org/obo/GAZ_00017432 -->

    <owl:NamedIndividual rdf:about="http://purl.obolibrary.org/obo/GAZ_00017432">
        <obo:RO_0001025 rdf:resource="http://purl.obolibrary.org/obo/GAZ_00017424"/>
        <obo:IAO_0000115>An island in the Main Group of the Bounty Islands.</obo:IAO_0000115>
        <oboInOwl:hasOBONamespace>GAZ</oboInOwl:hasOBONamespace>
        <oboInOwl:id>GAZ:00017432</oboInOwl:id>
        <rdfs:label>Penguin Island</rdfs:label>
    </owl:NamedIndividual>
    


    <!-- http://purl.obolibrary.org/obo/GAZ_00017433 -->

    <owl:NamedIndividual rdf:about="http://purl.obolibrary.org/obo/GAZ_00017433">
        <obo:RO_0001025 rdf:resource="http://purl.obolibrary.org/obo/GAZ_00017424"/>
        <obo:IAO_0000115>An island in the Main Group of the Bounty Islands.</obo:IAO_0000115>
        <oboInOwl:hasOBONamespace>GAZ</oboInOwl:hasOBONamespace>
        <oboInOwl:id>GAZ:00017433</oboInOwl:id>
        <rdfs:label>Ruatara Island</rdfs:label>
    </owl:NamedIndividual>
    


    <!-- http://purl.obolibrary.org/obo/GAZ_00017434 -->

    <owl:NamedIndividual rdf:about="http://purl.obolibrary.org/obo/GAZ_00017434">
        <obo:RO_0001025 rdf:resource="http://purl.obolibrary.org/obo/GAZ_00017422"/>
        <obo:IAO_0000115>An island in the Centre Group of the Bounty Islands.</obo:IAO_0000115>
        <oboInOwl:hasOBONamespace>GAZ</oboInOwl:hasOBONamespace>
        <oboInOwl:id>GAZ:00017434</oboInOwl:id>
        <rdfs:label>Castle Island</rdfs:label>
    </owl:NamedIndividual>
    


    <!-- http://purl.obolibrary.org/obo/GAZ_00017435 -->

    <owl:NamedIndividual rdf:about="http://purl.obolibrary.org/obo/GAZ_00017435">
        <obo:RO_0001025 rdf:resource="http://purl.obolibrary.org/obo/GAZ_00017422"/>
        <obo:IAO_0000115>An island in the Centre Group of the Bounty Islands.</obo:IAO_0000115>
        <oboInOwl:hasOBONamespace>GAZ</oboInOwl:hasOBONamespace>
        <oboInOwl:id>GAZ:00017435</oboInOwl:id>
        <rdfs:label>Funnel Island</rdfs:label>
    </owl:NamedIndividual>
    


    <!-- http://purl.obolibrary.org/obo/GAZ_00017436 -->

    <owl:NamedIndividual rdf:about="http://purl.obolibrary.org/obo/GAZ_00017436">
        <obo:RO_0001025 rdf:resource="http://purl.obolibrary.org/obo/GAZ_00017423"/>
        <obo:IAO_0000115>A small island in the East Group of the Bounty Islands.</obo:IAO_0000115>
        <oboInOwl:hasOBONamespace>GAZ</oboInOwl:hasOBONamespace>
        <oboInOwl:id>GAZ:00017436</oboInOwl:id>
        <rdfs:label>Molly Cap</rdfs:label>
    </owl:NamedIndividual>
    


    <!-- http://purl.obolibrary.org/obo/GAZ_00017437 -->

    <owl:NamedIndividual rdf:about="http://purl.obolibrary.org/obo/GAZ_00017437">
        <obo:RO_0001025 rdf:resource="http://purl.obolibrary.org/obo/GAZ_00017423"/>
        <obo:IAO_0000115>A rockin the East Group of the Bounty Islands.</obo:IAO_0000115>
        <oboInOwl:hasOBONamespace>GAZ</oboInOwl:hasOBONamespace>
        <oboInOwl:id>GAZ:00017437</oboInOwl:id>
        <rdfs:label>North Rock</rdfs:label>
    </owl:NamedIndividual>
    


    <!-- http://purl.obolibrary.org/obo/GAZ_00017438 -->

    <owl:NamedIndividual rdf:about="http://purl.obolibrary.org/obo/GAZ_00017438">
        <obo:RO_0001025 rdf:resource="http://purl.obolibrary.org/obo/GAZ_00007175"/>
        <obo:IAO_0000115>A subantarctic island located in New Zealand&apos;s Campbell Island group.</obo:IAO_0000115>
        <oboInOwl:hasOBONamespace>GAZ</oboInOwl:hasOBONamespace>
        <oboInOwl:id>GAZ:00017438</oboInOwl:id>
        <rdfs:label>Folly Island</rdfs:label>
    </owl:NamedIndividual>
    


    <!-- http://purl.obolibrary.org/obo/GAZ_00017439 -->

    <owl:NamedIndividual rdf:about="http://purl.obolibrary.org/obo/GAZ_00017439">
        <obo:RO_0001025 rdf:resource="http://purl.obolibrary.org/obo/GAZ_00007175"/>
        <obo:IAO_0000115>One of the islands surrounding Campbell Island, New Zealand. It is located 1 km south of Campbell Island and is the southernmost island of New Zealand. Jacquemart Island is a stack with an area of 19 ha, being about 750 m in length by 500 m in width and surrounded by precipitous cliffs at least 30 m high at their lowest.</obo:IAO_0000115>
        <oboInOwl:hasOBONamespace>GAZ</oboInOwl:hasOBONamespace>
        <oboInOwl:id>GAZ:00017439</oboInOwl:id>
        <rdfs:label>Jacquemart Island</rdfs:label>
    </owl:NamedIndividual>
    


    <!-- http://purl.obolibrary.org/obo/GAZ_00017440 -->

    <owl:NamedIndividual rdf:about="http://purl.obolibrary.org/obo/GAZ_00017440">
        <obo:RO_0001025 rdf:resource="http://purl.obolibrary.org/obo/GAZ_00007175"/>
        <obo:IAO_0000115>A remote, sub-Antarctic volcanic island of New Zealand and the main island of the Campbell Island group. It consists of 3 large peninsulas radiating in SE, NE and W directions.</obo:IAO_0000115>
        <oboInOwl:hasOBONamespace>GAZ</oboInOwl:hasOBONamespace>
        <oboInOwl:id>GAZ:00017440</oboInOwl:id>
        <rdfs:label>Campbell Island</rdfs:label>
    </owl:NamedIndividual>
    


    <!-- http://purl.obolibrary.org/obo/GAZ_00017441 -->

    <owl:NamedIndividual rdf:about="http://purl.obolibrary.org/obo/GAZ_00017441">
        <obo:RO_0001025 rdf:resource="http://purl.obolibrary.org/obo/GAZ_00007175"/>
        <obo:IAO_0000115>A sub-Antarctic 26 ha rock stack, lying 3 km west of Campbell Island and belonging to the Campbell Island group.</obo:IAO_0000115>
        <oboInOwl:hasOBONamespace>GAZ</oboInOwl:hasOBONamespace>
        <oboInOwl:id>GAZ:00017441</oboInOwl:id>
        <rdfs:label>Dent Island</rdfs:label>
    </owl:NamedIndividual>
    


    <!-- http://purl.obolibrary.org/obo/GAZ_00029928 -->

    <owl:NamedIndividual rdf:about="http://purl.obolibrary.org/obo/GAZ_00029928">
        <obo:RO_0001025 rdf:resource="http://purl.obolibrary.org/obo/GAZ_00008569"/>
        <obo:IAO_0000115>The northernmost district within New Zealand, consisting of the northern tip of the North Island.</obo:IAO_0000115>
        <oboInOwl:hasOBONamespace>GAZ</oboInOwl:hasOBONamespace>
        <oboInOwl:id>GAZ:00029928</oboInOwl:id>
        <rdfs:label>Far North District</rdfs:label>
    </owl:NamedIndividual>
    


    <!-- http://purl.obolibrary.org/obo/GAZ_00029929 -->

    <owl:NamedIndividual rdf:about="http://purl.obolibrary.org/obo/GAZ_00029929">
        <obo:RO_0001025 rdf:resource="http://purl.obolibrary.org/obo/GAZ_00008569"/>
        <oboInOwl:hasOBONamespace>GAZ</oboInOwl:hasOBONamespace>
        <oboInOwl:id>GAZ:00029929</oboInOwl:id>
        <rdfs:label>Kaipara District</rdfs:label>
    </owl:NamedIndividual>
    


    <!-- http://purl.obolibrary.org/obo/GAZ_00029930 -->

    <owl:NamedIndividual rdf:about="http://purl.obolibrary.org/obo/GAZ_00029930">
        <obo:RO_0001025 rdf:resource="http://purl.obolibrary.org/obo/GAZ_00004760"/>
        <oboInOwl:hasOBONamespace>GAZ</oboInOwl:hasOBONamespace>
        <oboInOwl:id>GAZ:00029930</oboInOwl:id>
        <rdfs:label>Rodney District</rdfs:label>
    </owl:NamedIndividual>
    


    <!-- http://purl.obolibrary.org/obo/GAZ_00029931 -->

    <owl:NamedIndividual rdf:about="http://purl.obolibrary.org/obo/GAZ_00029931">
        <obo:RO_0001025 rdf:resource="http://purl.obolibrary.org/obo/GAZ_00004760"/>
        <oboInOwl:hasOBONamespace>GAZ</oboInOwl:hasOBONamespace>
        <oboInOwl:id>GAZ:00029931</oboInOwl:id>
        <rdfs:label>Papakura District</rdfs:label>
    </owl:NamedIndividual>
    


    <!-- http://purl.obolibrary.org/obo/GAZ_00029932 -->

    <owl:NamedIndividual rdf:about="http://purl.obolibrary.org/obo/GAZ_00029932">
        <obo:RO_0001025 rdf:resource="http://purl.obolibrary.org/obo/GAZ_00004760"/>
        <obo:RO_0001025 rdf:resource="http://purl.obolibrary.org/obo/GAZ_00004781"/>
        <oboInOwl:hasOBONamespace>GAZ</oboInOwl:hasOBONamespace>
        <oboInOwl:id>GAZ:00029932</oboInOwl:id>
        <rdfs:label>Franklin District</rdfs:label>
    </owl:NamedIndividual>
    


    <!-- http://purl.obolibrary.org/obo/GAZ_00029933 -->

    <owl:NamedIndividual rdf:about="http://purl.obolibrary.org/obo/GAZ_00029933">
        <obo:RO_0001025 rdf:resource="http://purl.obolibrary.org/obo/GAZ_00004781"/>
        <oboInOwl:hasOBONamespace>GAZ</oboInOwl:hasOBONamespace>
        <oboInOwl:id>GAZ:00029933</oboInOwl:id>
        <rdfs:label>South Waikato District</rdfs:label>
    </owl:NamedIndividual>
    


    <!-- http://purl.obolibrary.org/obo/GAZ_00029934 -->

    <owl:NamedIndividual rdf:about="http://purl.obolibrary.org/obo/GAZ_00029934">
        <obo:RO_0001025 rdf:resource="http://purl.obolibrary.org/obo/GAZ_00004781"/>
        <oboInOwl:hasOBONamespace>GAZ</oboInOwl:hasOBONamespace>
        <oboInOwl:id>GAZ:00029934</oboInOwl:id>
        <rdfs:label>Matamata-Piako District</rdfs:label>
    </owl:NamedIndividual>
    


    <!-- http://purl.obolibrary.org/obo/GAZ_00029935 -->

    <owl:NamedIndividual rdf:about="http://purl.obolibrary.org/obo/GAZ_00029935">
        <obo:RO_0001025 rdf:resource="http://purl.obolibrary.org/obo/GAZ_00004781"/>
        <oboInOwl:hasOBONamespace>GAZ</oboInOwl:hasOBONamespace>
        <oboInOwl:id>GAZ:00029935</oboInOwl:id>
        <rdfs:label>Waipa District</rdfs:label>
    </owl:NamedIndividual>
    


    <!-- http://purl.obolibrary.org/obo/GAZ_00029936 -->

    <owl:NamedIndividual rdf:about="http://purl.obolibrary.org/obo/GAZ_00029936">
        <obo:RO_0001025 rdf:resource="http://purl.obolibrary.org/obo/GAZ_00004781"/>
        <oboInOwl:hasOBONamespace>GAZ</oboInOwl:hasOBONamespace>
        <oboInOwl:id>GAZ:00029936</oboInOwl:id>
        <rdfs:label>Waikato District</rdfs:label>
    </owl:NamedIndividual>
    


    <!-- http://purl.obolibrary.org/obo/GAZ_00029937 -->

    <owl:NamedIndividual rdf:about="http://purl.obolibrary.org/obo/GAZ_00029937">
        <obo:RO_0001025 rdf:resource="http://purl.obolibrary.org/obo/GAZ_00004781"/>
        <oboInOwl:hasOBONamespace>GAZ</oboInOwl:hasOBONamespace>
        <oboInOwl:id>GAZ:00029937</oboInOwl:id>
        <rdfs:label>Thames-Coromandel District</rdfs:label>
    </owl:NamedIndividual>
    


    <!-- http://purl.obolibrary.org/obo/GAZ_00029938 -->

    <owl:NamedIndividual rdf:about="http://purl.obolibrary.org/obo/GAZ_00029938">
        <obo:RO_0001025 rdf:resource="http://purl.obolibrary.org/obo/GAZ_00004781"/>
        <oboInOwl:hasOBONamespace>GAZ</oboInOwl:hasOBONamespace>
        <oboInOwl:id>GAZ:00029938</oboInOwl:id>
        <rdfs:label>Waitomo District</rdfs:label>
    </owl:NamedIndividual>
    


    <!-- http://purl.obolibrary.org/obo/GAZ_00029939 -->

    <owl:NamedIndividual rdf:about="http://purl.obolibrary.org/obo/GAZ_00029939">
        <obo:RO_0001025 rdf:resource="http://purl.obolibrary.org/obo/GAZ_00004781"/>
        <oboInOwl:hasOBONamespace>GAZ</oboInOwl:hasOBONamespace>
        <oboInOwl:id>GAZ:00029939</oboInOwl:id>
        <rdfs:label>Hauraki District</rdfs:label>
    </owl:NamedIndividual>
    


    <!-- http://purl.obolibrary.org/obo/GAZ_00029940 -->

    <owl:NamedIndividual rdf:about="http://purl.obolibrary.org/obo/GAZ_00029940">
        <obo:RO_0001025 rdf:resource="http://purl.obolibrary.org/obo/GAZ_00008564"/>
        <oboInOwl:hasOBONamespace>GAZ</oboInOwl:hasOBONamespace>
        <oboInOwl:id>GAZ:00029940</oboInOwl:id>
        <rdfs:label>Stratford District</rdfs:label>
    </owl:NamedIndividual>
    


    <!-- http://purl.obolibrary.org/obo/GAZ_00029941 -->

    <owl:NamedIndividual rdf:about="http://purl.obolibrary.org/obo/GAZ_00029941">
        <obo:RO_0001025 rdf:resource="http://purl.obolibrary.org/obo/GAZ_00004781"/>
        <oboInOwl:hasOBONamespace>GAZ</oboInOwl:hasOBONamespace>
        <oboInOwl:id>GAZ:00029941</oboInOwl:id>
        <rdfs:label>Otorohanga District</rdfs:label>
    </owl:NamedIndividual>
    


    <!-- http://purl.obolibrary.org/obo/GAZ_00029942 -->

    <owl:NamedIndividual rdf:about="http://purl.obolibrary.org/obo/GAZ_00029942">
        <obo:RO_0001025 rdf:resource="http://purl.obolibrary.org/obo/GAZ_00007723"/>
        <oboInOwl:hasOBONamespace>GAZ</oboInOwl:hasOBONamespace>
        <oboInOwl:id>GAZ:00029942</oboInOwl:id>
        <rdfs:label>Western Bay of Plenty District</rdfs:label>
    </owl:NamedIndividual>
    


    <!-- http://purl.obolibrary.org/obo/GAZ_00029943 -->

    <owl:NamedIndividual rdf:about="http://purl.obolibrary.org/obo/GAZ_00029943">
        <obo:RO_0001025 rdf:resource="http://purl.obolibrary.org/obo/GAZ_00007723"/>
        <oboInOwl:hasOBONamespace>GAZ</oboInOwl:hasOBONamespace>
        <oboInOwl:id>GAZ:00029943</oboInOwl:id>
        <rdfs:label>Opotiki District</rdfs:label>
    </owl:NamedIndividual>
    


    <!-- http://purl.obolibrary.org/obo/GAZ_00029944 -->

    <owl:NamedIndividual rdf:about="http://purl.obolibrary.org/obo/GAZ_00029944">
        <obo:RO_0001025 rdf:resource="http://purl.obolibrary.org/obo/GAZ_00007723"/>
        <oboInOwl:hasOBONamespace>GAZ</oboInOwl:hasOBONamespace>
        <oboInOwl:id>GAZ:00029944</oboInOwl:id>
        <rdfs:label>Kawerau District</rdfs:label>
    </owl:NamedIndividual>
    


    <!-- http://purl.obolibrary.org/obo/GAZ_00029945 -->

    <owl:NamedIndividual rdf:about="http://purl.obolibrary.org/obo/GAZ_00029945">
        <obo:RO_0001025 rdf:resource="http://purl.obolibrary.org/obo/GAZ_00010256"/>
        <oboInOwl:hasOBONamespace>GAZ</oboInOwl:hasOBONamespace>
        <oboInOwl:id>GAZ:00029945</oboInOwl:id>
        <rdfs:label>Wairoa District</rdfs:label>
    </owl:NamedIndividual>
    


    <!-- http://purl.obolibrary.org/obo/GAZ_00029946 -->

    <owl:NamedIndividual rdf:about="http://purl.obolibrary.org/obo/GAZ_00029946">
        <obo:RO_0001025 rdf:resource="http://purl.obolibrary.org/obo/GAZ_00010256"/>
        <oboInOwl:hasOBONamespace>GAZ</oboInOwl:hasOBONamespace>
        <oboInOwl:id>GAZ:00029946</oboInOwl:id>
        <rdfs:label>Central Hawke&apos;s Bay District</rdfs:label>
    </owl:NamedIndividual>
    


    <!-- http://purl.obolibrary.org/obo/GAZ_00029947 -->

    <owl:NamedIndividual rdf:about="http://purl.obolibrary.org/obo/GAZ_00029947">
        <obo:RO_0001025 rdf:resource="http://purl.obolibrary.org/obo/GAZ_00010256"/>
        <oboInOwl:hasOBONamespace>GAZ</oboInOwl:hasOBONamespace>
        <oboInOwl:id>GAZ:00029947</oboInOwl:id>
        <rdfs:label>Hastings District</rdfs:label>
    </owl:NamedIndividual>
    


    <!-- http://purl.obolibrary.org/obo/GAZ_00029948 -->

    <owl:NamedIndividual rdf:about="http://purl.obolibrary.org/obo/GAZ_00029948">
        <obo:RO_0001025 rdf:resource="http://purl.obolibrary.org/obo/GAZ_00010256"/>
        <obo:IAO_0000115>A port city in Hawke&apos;s Bay, New Zealand.</obo:IAO_0000115>
        <oboInOwl:hasOBONamespace>GAZ</oboInOwl:hasOBONamespace>
        <oboInOwl:id>GAZ:00029948</oboInOwl:id>
        <rdfs:label>Napier City</rdfs:label>
    </owl:NamedIndividual>
    


    <!-- http://purl.obolibrary.org/obo/GAZ_00029949 -->

    <owl:NamedIndividual rdf:about="http://purl.obolibrary.org/obo/GAZ_00029949">
        <obo:RO_0001025 rdf:resource="http://purl.obolibrary.org/obo/GAZ_00008564"/>
        <oboInOwl:hasOBONamespace>GAZ</oboInOwl:hasOBONamespace>
        <oboInOwl:id>GAZ:00029949</oboInOwl:id>
        <rdfs:label>New Plymouth District</rdfs:label>
    </owl:NamedIndividual>
    


    <!-- http://purl.obolibrary.org/obo/GAZ_00029950 -->

    <owl:NamedIndividual rdf:about="http://purl.obolibrary.org/obo/GAZ_00029950">
        <obo:RO_0001025 rdf:resource="http://purl.obolibrary.org/obo/GAZ_00008564"/>
        <oboInOwl:hasOBONamespace>GAZ</oboInOwl:hasOBONamespace>
        <oboInOwl:id>GAZ:00029950</oboInOwl:id>
        <rdfs:label>South Taranaki District</rdfs:label>
    </owl:NamedIndividual>
    


    <!-- http://purl.obolibrary.org/obo/GAZ_00029951 -->

    <owl:NamedIndividual rdf:about="http://purl.obolibrary.org/obo/GAZ_00029951">
        <obo:RO_0001025 rdf:resource="http://purl.obolibrary.org/obo/GAZ_00004772"/>
        <oboInOwl:hasOBONamespace>GAZ</oboInOwl:hasOBONamespace>
        <oboInOwl:id>GAZ:00029951</oboInOwl:id>
        <rdfs:label>Rangitikei District</rdfs:label>
    </owl:NamedIndividual>
    


    <!-- http://purl.obolibrary.org/obo/GAZ_00029952 -->

    <owl:NamedIndividual rdf:about="http://purl.obolibrary.org/obo/GAZ_00029952">
        <rdf:type rdf:resource="http://purl.obolibrary.org/obo/ENVO_00000004"/>
        <obo:RO_0001025 rdf:resource="http://purl.obolibrary.org/obo/GAZ_00004772"/>
        <obo:IAO_0000115>A district on the west coast of the North Island of New Zealand. Located north of Wellington and Kapiti, the district stretches from slightly north of the town of Otaki in the south to just south of Himatangi in the north, and from the coast to the summit of the Tararua Ranges.</obo:IAO_0000115>
        <oboInOwl:hasOBONamespace>GAZ</oboInOwl:hasOBONamespace>
        <oboInOwl:id>GAZ:00029952</oboInOwl:id>
        <rdfs:label>Horowhenua District</rdfs:label>
    </owl:NamedIndividual>
    


    <!-- http://purl.obolibrary.org/obo/GAZ_00029953 -->

    <owl:NamedIndividual rdf:about="http://purl.obolibrary.org/obo/GAZ_00029953">
        <obo:RO_0001025 rdf:resource="http://purl.obolibrary.org/obo/GAZ_00004772"/>
        <obo:IAO_0000115>A territorial authority near the centre of New Zealand&apos;s North Island.</obo:IAO_0000115>
        <oboInOwl:hasOBONamespace>GAZ</oboInOwl:hasOBONamespace>
        <oboInOwl:id>GAZ:00029953</oboInOwl:id>
        <rdfs:label>Ruapehu District</rdfs:label>
    </owl:NamedIndividual>
    


    <!-- http://purl.obolibrary.org/obo/GAZ_00029954 -->

    <owl:NamedIndividual rdf:about="http://purl.obolibrary.org/obo/GAZ_00029954">
        <obo:RO_0001025 rdf:resource="http://purl.obolibrary.org/obo/GAZ_00008565"/>
        <oboInOwl:hasOBONamespace>GAZ</oboInOwl:hasOBONamespace>
        <oboInOwl:id>GAZ:00029954</oboInOwl:id>
        <rdfs:label>Carterton District</rdfs:label>
    </owl:NamedIndividual>
    


    <!-- http://purl.obolibrary.org/obo/GAZ_00029955 -->

    <owl:NamedIndividual rdf:about="http://purl.obolibrary.org/obo/GAZ_00029955">
        <obo:RO_0001025 rdf:resource="http://purl.obolibrary.org/obo/GAZ_00008565"/>
        <oboInOwl:hasOBONamespace>GAZ</oboInOwl:hasOBONamespace>
        <oboInOwl:id>GAZ:00029955</oboInOwl:id>
        <rdfs:label>South Wairarapa District</rdfs:label>
    </owl:NamedIndividual>
    


    <!-- http://purl.obolibrary.org/obo/GAZ_00029956 -->

    <owl:NamedIndividual rdf:about="http://purl.obolibrary.org/obo/GAZ_00029956">
        <obo:RO_0001025 rdf:resource="http://purl.obolibrary.org/obo/GAZ_00008565"/>
        <oboInOwl:hasOBONamespace>GAZ</oboInOwl:hasOBONamespace>
        <oboInOwl:id>GAZ:00029956</oboInOwl:id>
        <rdfs:label>Masterton District</rdfs:label>
    </owl:NamedIndividual>
    


    <!-- http://purl.obolibrary.org/obo/GAZ_00029957 -->

    <owl:NamedIndividual rdf:about="http://purl.obolibrary.org/obo/GAZ_00029957">
        <obo:RO_0001025 rdf:resource="http://purl.obolibrary.org/obo/GAZ_00008565"/>
        <obo:IAO_0000115>A populated place. A city in the Wellington Region of New Zealand, 20 km north of the city of Wellington. It almost completely surrounds Porirua Harbour at the southern end of the Kapiti Coast.</obo:IAO_0000115>
        <oboInOwl:hasOBONamespace>GAZ</oboInOwl:hasOBONamespace>
        <oboInOwl:id>GAZ:00029957</oboInOwl:id>
        <rdfs:label>Porirua City</rdfs:label>
    </owl:NamedIndividual>
    


    <!-- http://purl.obolibrary.org/obo/GAZ_00029958 -->

    <owl:NamedIndividual rdf:about="http://purl.obolibrary.org/obo/GAZ_00029958">
        <obo:RO_0001025 rdf:resource="http://purl.obolibrary.org/obo/GAZ_00008565"/>
        <oboInOwl:hasOBONamespace>GAZ</oboInOwl:hasOBONamespace>
        <oboInOwl:id>GAZ:00029958</oboInOwl:id>
        <rdfs:label>Kapiti Coast District</rdfs:label>
    </owl:NamedIndividual>
    


    <!-- http://purl.obolibrary.org/obo/GAZ_00029959 -->

    <owl:NamedIndividual rdf:about="http://purl.obolibrary.org/obo/GAZ_00029959">
        <obo:RO_0001025 rdf:resource="http://purl.obolibrary.org/obo/GAZ_00004777"/>
        <obo:IAO_0000115>An administrative region in the West Coast region of New Zealand. It covers Westport, Karamea, Reefton and Inangahua Junction.</obo:IAO_0000115>
        <oboInOwl:hasOBONamespace>GAZ</oboInOwl:hasOBONamespace>
        <oboInOwl:id>GAZ:00029959</oboInOwl:id>
        <rdfs:label>Buller District</rdfs:label>
    </owl:NamedIndividual>
    


    <!-- http://purl.obolibrary.org/obo/GAZ_00029960 -->

    <owl:NamedIndividual rdf:about="http://purl.obolibrary.org/obo/GAZ_00029960">
        <obo:RO_0001025 rdf:resource="http://purl.obolibrary.org/obo/GAZ_00004777"/>
        <oboInOwl:hasOBONamespace>GAZ</oboInOwl:hasOBONamespace>
        <oboInOwl:id>GAZ:00029960</oboInOwl:id>
        <rdfs:label>Grey District</rdfs:label>
    </owl:NamedIndividual>
    


    <!-- http://purl.obolibrary.org/obo/GAZ_00029961 -->

    <owl:NamedIndividual rdf:about="http://purl.obolibrary.org/obo/GAZ_00029961">
        <obo:RO_0001025 rdf:resource="http://purl.obolibrary.org/obo/GAZ_00008562"/>
        <oboInOwl:hasOBONamespace>GAZ</oboInOwl:hasOBONamespace>
        <oboInOwl:id>GAZ:00029961</oboInOwl:id>
        <rdfs:label>Waimate District</rdfs:label>
    </owl:NamedIndividual>
    


    <!-- http://purl.obolibrary.org/obo/GAZ_00029962 -->

    <owl:NamedIndividual rdf:about="http://purl.obolibrary.org/obo/GAZ_00029962">
        <obo:RO_0001025 rdf:resource="http://purl.obolibrary.org/obo/GAZ_00008562"/>
        <oboInOwl:hasOBONamespace>GAZ</oboInOwl:hasOBONamespace>
        <oboInOwl:id>GAZ:00029962</oboInOwl:id>
        <rdfs:label>Mackenzie District</rdfs:label>
    </owl:NamedIndividual>
    


    <!-- http://purl.obolibrary.org/obo/GAZ_00029963 -->

    <owl:NamedIndividual rdf:about="http://purl.obolibrary.org/obo/GAZ_00029963">
        <obo:RO_0001025 rdf:resource="http://purl.obolibrary.org/obo/GAZ_00008562"/>
        <oboInOwl:hasOBONamespace>GAZ</oboInOwl:hasOBONamespace>
        <oboInOwl:id>GAZ:00029963</oboInOwl:id>
        <rdfs:label>Waimakariri District</rdfs:label>
    </owl:NamedIndividual>
    


    <!-- http://purl.obolibrary.org/obo/GAZ_00029964 -->

    <owl:NamedIndividual rdf:about="http://purl.obolibrary.org/obo/GAZ_00029964">
        <obo:RO_0001025 rdf:resource="http://purl.obolibrary.org/obo/GAZ_00008562"/>
        <oboInOwl:hasOBONamespace>GAZ</oboInOwl:hasOBONamespace>
        <oboInOwl:id>GAZ:00029964</oboInOwl:id>
        <rdfs:label>Hurunui District</rdfs:label>
    </owl:NamedIndividual>
    


    <!-- http://purl.obolibrary.org/obo/GAZ_00029965 -->

    <owl:NamedIndividual rdf:about="http://purl.obolibrary.org/obo/GAZ_00029965">
        <obo:RO_0001025 rdf:resource="http://purl.obolibrary.org/obo/GAZ_00008562"/>
        <oboInOwl:hasOBONamespace>GAZ</oboInOwl:hasOBONamespace>
        <oboInOwl:id>GAZ:00029965</oboInOwl:id>
        <rdfs:label>Kaikoura District</rdfs:label>
    </owl:NamedIndividual>
    


    <!-- http://purl.obolibrary.org/obo/GAZ_00029966 -->

    <owl:NamedIndividual rdf:about="http://purl.obolibrary.org/obo/GAZ_00029966">
        <obo:RO_0001025 rdf:resource="http://purl.obolibrary.org/obo/GAZ_00004767"/>
        <oboInOwl:hasOBONamespace>GAZ</oboInOwl:hasOBONamespace>
        <oboInOwl:id>GAZ:00029966</oboInOwl:id>
        <rdfs:label>Clutha District</rdfs:label>
    </owl:NamedIndividual>
    


    <!-- http://purl.obolibrary.org/obo/GAZ_00029967 -->

    <owl:NamedIndividual rdf:about="http://purl.obolibrary.org/obo/GAZ_00029967">
        <obo:RO_0001025 rdf:resource="http://purl.obolibrary.org/obo/GAZ_00004767"/>
        <oboInOwl:hasOBONamespace>GAZ</oboInOwl:hasOBONamespace>
        <oboInOwl:id>GAZ:00029967</oboInOwl:id>
        <rdfs:label>Queenstown Lakes District</rdfs:label>
    </owl:NamedIndividual>
    


    <!-- http://purl.obolibrary.org/obo/GAZ_00029968 -->

    <owl:NamedIndividual rdf:about="http://purl.obolibrary.org/obo/GAZ_00029968">
        <obo:RO_0001025 rdf:resource="http://purl.obolibrary.org/obo/GAZ_00008572"/>
        <oboInOwl:hasOBONamespace>GAZ</oboInOwl:hasOBONamespace>
        <oboInOwl:id>GAZ:00029968</oboInOwl:id>
        <rdfs:label>Gore District</rdfs:label>
    </owl:NamedIndividual>
    


    <!-- http://purl.obolibrary.org/obo/GAZ_00030187 -->

    <owl:NamedIndividual rdf:about="http://purl.obolibrary.org/obo/GAZ_00030187">
        <obo:RO_0001025 rdf:resource="http://purl.obolibrary.org/obo/GAZ_00004767"/>
        <obo:IAO_0000115>The second longest river in New Zealand and flows south-southeast for 340 km through Central and South Otago to the Pacific Ocean, 75 km south west of Dunedin.</obo:IAO_0000115>
        <oboInOwl:hasOBONamespace>GAZ</oboInOwl:hasOBONamespace>
        <oboInOwl:id>GAZ:00030187</oboInOwl:id>
        <rdfs:label>The Cluther</rdfs:label>
    </owl:NamedIndividual>
    


    <!-- http://purl.obolibrary.org/obo/GAZ_00030188 -->

    <owl:NamedIndividual rdf:about="http://purl.obolibrary.org/obo/GAZ_00030188">
        <obo:RO_0001025 rdf:resource="http://purl.obolibrary.org/obo/GAZ_00030187"/>
        <oboInOwl:hasOBONamespace>GAZ</oboInOwl:hasOBONamespace>
        <oboInOwl:id>GAZ:00030188</oboInOwl:id>
        <rdfs:label>12 Mile Creek</rdfs:label>
    </owl:NamedIndividual>
    


    <!-- http://purl.obolibrary.org/obo/GAZ_00030189 -->

    <owl:NamedIndividual rdf:about="http://purl.obolibrary.org/obo/GAZ_00030189">
        <obo:RO_0001025 rdf:resource="http://purl.obolibrary.org/obo/GAZ_00008563"/>
        <obo:IAO_0000115>A national park located at the north end of the South Island of New Zealand. The park consists of forested, hilly country to the north of the valleys of the Takaka and Riwaka Rivers, and is bounded to the north by the waters of Golden Bay and Tasman Bay.</obo:IAO_0000115>
        <oboInOwl:hasOBONamespace>GAZ</oboInOwl:hasOBONamespace>
        <oboInOwl:id>GAZ:00030189</oboInOwl:id>
        <rdfs:label>Abel Tasman National Park</rdfs:label>
    </owl:NamedIndividual>
    


    <!-- http://purl.obolibrary.org/obo/GAZ_00030192 -->

    <owl:NamedIndividual rdf:about="http://purl.obolibrary.org/obo/GAZ_00030192">
        <obo:RO_0001025 rdf:resource="http://purl.obolibrary.org/obo/GAZ_00004767"/>
        <obo:IAO_0000115>A river in the Otago region of the South Island of New Zealand. The headwaters are on the eastern flanks of the Southern Alps. The river flows for 70 km through the southernmost part of the Mackenzie Basin before reaching Lake Benmore, one of the lakes in the Waitaki hydroelectric project. From there, the waters join with those of the Waitaki, which has its outflow in the Pacific Ocean.</obo:IAO_0000115>
        <oboInOwl:hasOBONamespace>GAZ</oboInOwl:hasOBONamespace>
        <oboInOwl:id>GAZ:00030192</oboInOwl:id>
        <rdfs:label>Ahuriri River</rdfs:label>
    </owl:NamedIndividual>
    


    <!-- http://purl.obolibrary.org/obo/GAZ_00030193 -->

    <owl:NamedIndividual rdf:about="http://purl.obolibrary.org/obo/GAZ_00030193">
        <rdf:type rdf:resource="http://purl.obolibrary.org/obo/ENVO_00000856"/>
        <obo:RO_0001025 rdf:resource="http://purl.obolibrary.org/obo/GAZ_00010246"/>
        <obo:IAO_0000115>A populated place. A town on Banks Peninsula in the Canterbury region of the South Island of New Zealand.</obo:IAO_0000115>
        <oboInOwl:hasOBONamespace>GAZ</oboInOwl:hasOBONamespace>
        <oboInOwl:id>GAZ:00030193</oboInOwl:id>
        <rdfs:label>Akaroa</rdfs:label>
    </owl:NamedIndividual>
    


    <!-- http://purl.obolibrary.org/obo/GAZ_00030194 -->

    <owl:NamedIndividual rdf:about="http://purl.obolibrary.org/obo/GAZ_00030194">
        <obo:RO_0001025 rdf:resource="http://purl.obolibrary.org/obo/GAZ_00004760"/>
        <obo:IAO_0000115>A populated place. A city in the Auckland region of New Zealand. North Shore is bounded by Rodney District to the north, Waitemata Harbour to the south and the Rangitoto Channel of the Hauraki Gulf to the east. The Auckland Harbour Bridge connects it to Auckland City on the south side of the Waitemata Harbour, while the Upper Harbour Bridge connects it to Waitakere in the west.</obo:IAO_0000115>
        <oboInOwl:hasOBONamespace>GAZ</oboInOwl:hasOBONamespace>
        <oboInOwl:id>GAZ:00030194</oboInOwl:id>
        <rdfs:label>North Shore City</rdfs:label>
    </owl:NamedIndividual>
    


    <!-- http://purl.obolibrary.org/obo/GAZ_00030195 -->

    <owl:NamedIndividual rdf:about="http://purl.obolibrary.org/obo/GAZ_00030195">
        <obo:RO_0001025 rdf:resource="http://purl.obolibrary.org/obo/GAZ_00030194"/>
        <oboInOwl:hasOBONamespace>GAZ</oboInOwl:hasOBONamespace>
        <oboInOwl:id>GAZ:00030195</oboInOwl:id>
        <rdfs:label>Albany</rdfs:label>
    </owl:NamedIndividual>
    


    <!-- http://purl.obolibrary.org/obo/GAZ_00030196 -->

    <owl:NamedIndividual rdf:about="http://purl.obolibrary.org/obo/GAZ_00030196">
        <obo:RO_0001025 rdf:resource="http://purl.obolibrary.org/obo/GAZ_00004767"/>
        <obo:IAO_0000115>A lake located in the Otago region of New Zealand, at an altitude of 300 m. Covering an area of 192 km2, it is New Zealand&apos;s fourth largest lake, and estimated to be more than 300 m deep.</obo:IAO_0000115>
        <oboInOwl:hasOBONamespace>GAZ</oboInOwl:hasOBONamespace>
        <oboInOwl:id>GAZ:00030196</oboInOwl:id>
        <rdfs:label>Lake Wanaka</rdfs:label>
    </owl:NamedIndividual>
    


    <!-- http://purl.obolibrary.org/obo/GAZ_00030197 -->

    <owl:NamedIndividual rdf:about="http://purl.obolibrary.org/obo/GAZ_00030197">
        <obo:RO_0001025 rdf:resource="http://purl.obolibrary.org/obo/GAZ_00029967"/>
        <oboInOwl:hasOBONamespace>GAZ</oboInOwl:hasOBONamespace>
        <oboInOwl:id>GAZ:00030197</oboInOwl:id>
        <rdfs:label>Albert Town</rdfs:label>
    </owl:NamedIndividual>
    


    <!-- http://purl.obolibrary.org/obo/GAZ_00030198 -->

    <owl:NamedIndividual rdf:about="http://purl.obolibrary.org/obo/GAZ_00030198">
        <obo:RO_0001025 rdf:resource="http://purl.obolibrary.org/obo/GAZ_00008569"/>
        <obo:IAO_0000115>A group of uninhabited volcanic islands off the east coast of the Northland Region of the North Island of New Zealand. They are located 50 km to the northeast of Whangarei, and lie 22 km offshore half way between Bream Head and Cape Brett.</obo:IAO_0000115>
        <oboInOwl:hasOBONamespace>GAZ</oboInOwl:hasOBONamespace>
        <oboInOwl:id>GAZ:00030198</oboInOwl:id>
        <rdfs:label>Poor Knights Islands</rdfs:label>
    </owl:NamedIndividual>
    


    <!-- http://purl.obolibrary.org/obo/GAZ_00030199 -->

    <owl:NamedIndividual rdf:about="http://purl.obolibrary.org/obo/GAZ_00030199">
        <obo:RO_0001025 rdf:resource="http://purl.obolibrary.org/obo/GAZ_00030198"/>
        <obo:IAO_0000115>One of the Poor Knights Islands.</obo:IAO_0000115>
        <oboInOwl:hasOBONamespace>GAZ</oboInOwl:hasOBONamespace>
        <oboInOwl:id>GAZ:00030199</oboInOwl:id>
        <rdfs:label>Aorangi Island</rdfs:label>
    </owl:NamedIndividual>
    


    <!-- http://purl.obolibrary.org/obo/GAZ_00030200 -->

    <owl:NamedIndividual rdf:about="http://purl.obolibrary.org/obo/GAZ_00030200">
        <obo:RO_0001025 rdf:resource="http://purl.obolibrary.org/obo/GAZ_00030198"/>
        <obo:IAO_0000115>One of the Poor Knights Islands.</obo:IAO_0000115>
        <oboInOwl:hasOBONamespace>GAZ</oboInOwl:hasOBONamespace>
        <oboInOwl:id>GAZ:00030200</oboInOwl:id>
        <rdfs:label>Tawhiti Rahi</rdfs:label>
    </owl:NamedIndividual>
    


    <!-- http://purl.obolibrary.org/obo/GAZ_00030201 -->

    <owl:NamedIndividual rdf:about="http://purl.obolibrary.org/obo/GAZ_00030201">
        <obo:RO_0001025 rdf:resource="http://purl.obolibrary.org/obo/GAZ_00030198"/>
        <obo:IAO_0000115>One of the Poor Knights Islands.</obo:IAO_0000115>
        <oboInOwl:hasOBONamespace>GAZ</oboInOwl:hasOBONamespace>
        <oboInOwl:id>GAZ:00030201</oboInOwl:id>
        <rdfs:label>Motu Kapiti</rdfs:label>
    </owl:NamedIndividual>
    


    <!-- http://purl.obolibrary.org/obo/GAZ_00030202 -->

    <owl:NamedIndividual rdf:about="http://purl.obolibrary.org/obo/GAZ_00030202">
        <obo:RO_0001025 rdf:resource="http://purl.obolibrary.org/obo/GAZ_00004765"/>
        <obo:IAO_0000115>An inlet of the Tasman Sea located near the base of the North Auckland Peninsula on the western side of the North Island of New Zealand.</obo:IAO_0000115>
        <oboInOwl:hasOBONamespace>GAZ</oboInOwl:hasOBONamespace>
        <oboInOwl:id>GAZ:00030202</oboInOwl:id>
        <rdfs:label>Kaipara Harbour</rdfs:label>
    </owl:NamedIndividual>
    


    <!-- http://purl.obolibrary.org/obo/GAZ_00030203 -->

    <owl:NamedIndividual rdf:about="http://purl.obolibrary.org/obo/GAZ_00030203">
        <obo:RO_0001025 rdf:resource="http://purl.obolibrary.org/obo/GAZ_00030202"/>
        <obo:IAO_0000115>Cliffs.</obo:IAO_0000115>
        <oboInOwl:hasOBONamespace>GAZ</oboInOwl:hasOBONamespace>
        <oboInOwl:id>GAZ:00030203</oboInOwl:id>
        <rdfs:label>Aotea Cliffs</rdfs:label>
    </owl:NamedIndividual>
    


    <!-- http://purl.obolibrary.org/obo/GAZ_00030204 -->

    <owl:NamedIndividual rdf:about="http://purl.obolibrary.org/obo/GAZ_00030204">
        <obo:RO_0001025 rdf:resource="http://purl.obolibrary.org/obo/GAZ_00046925"/>
        <obo:IAO_0000115>A small island located in the Marlborough Sounds, at the north east tip of the South Island of New Zealand. The island has a land area of 75 km2. Queen Charlotte Sound defines its western side, while to the south lies Tory Channel, which is on the sea route from Wellington in the North Island to Picton.</obo:IAO_0000115>
        <oboInOwl:hasOBONamespace>GAZ</oboInOwl:hasOBONamespace>
        <oboInOwl:id>GAZ:00030204</oboInOwl:id>
        <rdfs:label>Arapawa Island</rdfs:label>
    </owl:NamedIndividual>
    


    <!-- http://purl.obolibrary.org/obo/GAZ_00030205 -->

    <owl:NamedIndividual rdf:about="http://purl.obolibrary.org/obo/GAZ_00030205">
        <obo:RO_0001025 rdf:resource="http://purl.obolibrary.org/obo/GAZ_00007178"/>
        <oboInOwl:hasOBONamespace>GAZ</oboInOwl:hasOBONamespace>
        <oboInOwl:id>GAZ:00030205</oboInOwl:id>
        <rdfs:label>Archway Island</rdfs:label>
    </owl:NamedIndividual>
    


    <!-- http://purl.obolibrary.org/obo/GAZ_00030206 -->

    <owl:NamedIndividual rdf:about="http://purl.obolibrary.org/obo/GAZ_00030206">
        <obo:RO_0001025 rdf:resource="http://purl.obolibrary.org/obo/GAZ_00007178"/>
        <oboInOwl:hasOBONamespace>GAZ</oboInOwl:hasOBONamespace>
        <oboInOwl:id>GAZ:00030206</oboInOwl:id>
        <rdfs:label>King Group</rdfs:label>
    </owl:NamedIndividual>
    


    <!-- http://purl.obolibrary.org/obo/GAZ_00030207 -->

    <owl:NamedIndividual rdf:about="http://purl.obolibrary.org/obo/GAZ_00030207">
        <obo:RO_0001025 rdf:resource="http://purl.obolibrary.org/obo/GAZ_00007178"/>
        <oboInOwl:hasOBONamespace>GAZ</oboInOwl:hasOBONamespace>
        <oboInOwl:id>GAZ:00030207</oboInOwl:id>
        <rdfs:label>Southwest Group</rdfs:label>
    </owl:NamedIndividual>
    


    <!-- http://purl.obolibrary.org/obo/GAZ_00030208 -->

    <owl:NamedIndividual rdf:about="http://purl.obolibrary.org/obo/GAZ_00030208">
        <obo:RO_0001025 rdf:resource="http://purl.obolibrary.org/obo/GAZ_00030207"/>
        <oboInOwl:hasOBONamespace>GAZ</oboInOwl:hasOBONamespace>
        <oboInOwl:id>GAZ:00030208</oboInOwl:id>
        <rdfs:label>South West Island</rdfs:label>
    </owl:NamedIndividual>
    


    <!-- http://purl.obolibrary.org/obo/GAZ_00030209 -->

    <owl:NamedIndividual rdf:about="http://purl.obolibrary.org/obo/GAZ_00030209">
        <obo:RO_0001025 rdf:resource="http://purl.obolibrary.org/obo/GAZ_00030207"/>
        <oboInOwl:hasOBONamespace>GAZ</oboInOwl:hasOBONamespace>
        <oboInOwl:id>GAZ:00030209</oboInOwl:id>
        <rdfs:label>West Island</rdfs:label>
    </owl:NamedIndividual>
    


    <!-- http://purl.obolibrary.org/obo/GAZ_00030210 -->

    <owl:NamedIndividual rdf:about="http://purl.obolibrary.org/obo/GAZ_00030210">
        <obo:RO_0001025 rdf:resource="http://purl.obolibrary.org/obo/GAZ_00030207"/>
        <oboInOwl:hasOBONamespace>GAZ</oboInOwl:hasOBONamespace>
        <oboInOwl:id>GAZ:00030210</oboInOwl:id>
        <rdfs:label>The Princes Islands</rdfs:label>
    </owl:NamedIndividual>
    


    <!-- http://purl.obolibrary.org/obo/GAZ_00030211 -->

    <owl:NamedIndividual rdf:about="http://purl.obolibrary.org/obo/GAZ_00030211">
        <obo:RO_0001025 rdf:resource="http://purl.obolibrary.org/obo/GAZ_00030206"/>
        <oboInOwl:hasOBONamespace>GAZ</oboInOwl:hasOBONamespace>
        <oboInOwl:id>GAZ:00030211</oboInOwl:id>
        <rdfs:label>North East Island</rdfs:label>
    </owl:NamedIndividual>
    


    <!-- http://purl.obolibrary.org/obo/GAZ_00030212 -->

    <owl:NamedIndividual rdf:about="http://purl.obolibrary.org/obo/GAZ_00030212">
        <obo:RO_0001025 rdf:resource="http://purl.obolibrary.org/obo/GAZ_00030206"/>
        <oboInOwl:hasOBONamespace>GAZ</oboInOwl:hasOBONamespace>
        <oboInOwl:id>GAZ:00030212</oboInOwl:id>
        <rdfs:label>Farmers Rocks</rdfs:label>
    </owl:NamedIndividual>
    


    <!-- http://purl.obolibrary.org/obo/GAZ_00030213 -->

    <owl:NamedIndividual rdf:about="http://purl.obolibrary.org/obo/GAZ_00030213">
        <obo:RO_0001025 rdf:resource="http://purl.obolibrary.org/obo/GAZ_00030206"/>
        <oboInOwl:hasOBONamespace>GAZ</oboInOwl:hasOBONamespace>
        <oboInOwl:id>GAZ:00030213</oboInOwl:id>
        <rdfs:label>Great Island</rdfs:label>
    </owl:NamedIndividual>
    


    <!-- http://purl.obolibrary.org/obo/GAZ_00030214 -->

    <owl:NamedIndividual rdf:about="http://purl.obolibrary.org/obo/GAZ_00030214">
        <obo:RO_0001025 rdf:resource="http://purl.obolibrary.org/obo/GAZ_00004760"/>
        <obo:IAO_0000115>A peninsula located in the northern North Island of New Zealand, close to the base of the North Auckland Peninsula. The peninsula stretches east for 11 km into the waters of the Hauraki Gulf to the north of East Coast Bays. The island of Tiritiri Matangi lies three km off its eastern tip. The town of Whangaparaoa sits on the peninsula&apos;s southwestern shore, and is regarded as the start of the section of coastline known as the Hibiscus Coast.</obo:IAO_0000115>
        <oboInOwl:hasOBONamespace>GAZ</oboInOwl:hasOBONamespace>
        <oboInOwl:id>GAZ:00030214</oboInOwl:id>
        <rdfs:label>Whangaparaoa Peninsula</rdfs:label>
    </owl:NamedIndividual>
    


    <!-- http://purl.obolibrary.org/obo/GAZ_00030215 -->

    <owl:NamedIndividual rdf:about="http://purl.obolibrary.org/obo/GAZ_00030215">
        <obo:RO_0001025 rdf:resource="http://purl.obolibrary.org/obo/GAZ_00030214"/>
        <obo:IAO_0000115>A bay to the N of the Whangaparoa Peninsula.</obo:IAO_0000115>
        <oboInOwl:hasOBONamespace>GAZ</oboInOwl:hasOBONamespace>
        <oboInOwl:id>GAZ:00030215</oboInOwl:id>
        <rdfs:label>Army Bay</rdfs:label>
    </owl:NamedIndividual>
    


    <!-- http://purl.obolibrary.org/obo/GAZ_00030216 -->

    <owl:NamedIndividual rdf:about="http://purl.obolibrary.org/obo/GAZ_00030216">
        <obo:RO_0001025 rdf:resource="http://purl.obolibrary.org/obo/GAZ_00030214"/>
        <oboInOwl:hasOBONamespace>GAZ</oboInOwl:hasOBONamespace>
        <oboInOwl:id>GAZ:00030216</oboInOwl:id>
        <rdfs:label>Whangaparaoa</rdfs:label>
    </owl:NamedIndividual>
    


    <!-- http://purl.obolibrary.org/obo/GAZ_00030217 -->

    <owl:NamedIndividual rdf:about="http://purl.obolibrary.org/obo/GAZ_00030217">
        <obo:RO_0001025 rdf:resource="http://purl.obolibrary.org/obo/GAZ_00004764"/>
        <obo:IAO_0000115>A mountain range which runs along the western side of the South Island of New Zealand. It forms a natural dividing range along the entire length of the South Island. The term &quot;Southern Alps&quot; generally refers to the entire range, although separate names are given to many of the smaller ranges that form part of it.</obo:IAO_0000115>
        <oboInOwl:hasOBONamespace>GAZ</oboInOwl:hasOBONamespace>
        <oboInOwl:id>GAZ:00030217</oboInOwl:id>
        <rdfs:label>Southern Alps</rdfs:label>
    </owl:NamedIndividual>
    


    <!-- http://purl.obolibrary.org/obo/GAZ_00030218 -->

    <owl:NamedIndividual rdf:about="http://purl.obolibrary.org/obo/GAZ_00030218">
        <obo:RO_0001025 rdf:resource="http://purl.obolibrary.org/obo/GAZ_00030217"/>
        <obo:IAO_0000115>A mountain pass in the Southern Alps of the South Island of New Zealand. It marks part of the boundary between Westland and Canterbury, 140 km from Christchurch and 95 km from Greymouth. The pass lies in a saddle between the valleys of the Otira River, a tributary of the Taramakau in the west and the Bealey River in the east.</obo:IAO_0000115>
        <oboInOwl:hasOBONamespace>GAZ</oboInOwl:hasOBONamespace>
        <oboInOwl:id>GAZ:00030218</oboInOwl:id>
        <rdfs:label>Arthur&apos;s Pass</rdfs:label>
    </owl:NamedIndividual>
    


    <!-- http://purl.obolibrary.org/obo/GAZ_00030219 -->

    <owl:NamedIndividual rdf:about="http://purl.obolibrary.org/obo/GAZ_00030219">
        <obo:RO_0001025 rdf:resource="http://purl.obolibrary.org/obo/GAZ_00008562"/>
        <obo:IAO_0000115>A river located in Canterbury, New Zealand. It flows generally southeastwards for 65 km before entering the Pacific Ocean at Pegasus Bay north of Christchurch. Though the lower reaches of the river are braided, part of the upper river flows through a canyon known as the Ashley Gorge.</obo:IAO_0000115>
        <oboInOwl:hasOBONamespace>GAZ</oboInOwl:hasOBONamespace>
        <oboInOwl:id>GAZ:00030219</oboInOwl:id>
        <rdfs:label>Ashley River</rdfs:label>
    </owl:NamedIndividual>
    


    <!-- http://purl.obolibrary.org/obo/GAZ_00030220 -->

    <owl:NamedIndividual rdf:about="http://purl.obolibrary.org/obo/GAZ_00030220">
        <obo:RO_0001025 rdf:resource="http://purl.obolibrary.org/obo/GAZ_00030219"/>
        <obo:IAO_0000115>A river gorge of the Ashley River in Canterbury, New Zealand.</obo:IAO_0000115>
        <oboInOwl:hasOBONamespace>GAZ</oboInOwl:hasOBONamespace>
        <oboInOwl:id>GAZ:00030220</oboInOwl:id>
        <rdfs:label>Ashley Gorge</rdfs:label>
    </owl:NamedIndividual>
    


    <!-- http://purl.obolibrary.org/obo/GAZ_00030221 -->

    <owl:NamedIndividual rdf:about="http://purl.obolibrary.org/obo/GAZ_00030221">
        <obo:RO_0001025 rdf:resource="http://purl.obolibrary.org/obo/GAZ_00009534"/>
        <obo:IAO_0000115>A suburb located in Auckland, New Zealand. It is located nine km to the east of the city centre, close to the waters of the Tamaki River.</obo:IAO_0000115>
        <oboInOwl:hasOBONamespace>GAZ</oboInOwl:hasOBONamespace>
        <oboInOwl:id>GAZ:00030221</oboInOwl:id>
        <rdfs:label>Glen Innes</rdfs:label>
    </owl:NamedIndividual>
    


    <!-- http://purl.obolibrary.org/obo/GAZ_00030222 -->

    <owl:NamedIndividual rdf:about="http://purl.obolibrary.org/obo/GAZ_00030222">
        <obo:RO_0001025 rdf:resource="http://purl.obolibrary.org/obo/GAZ_00004760"/>
        <obo:IAO_0000115>A 182 metre volcanic peak located in Auckland, New Zealand.</obo:IAO_0000115>
        <oboInOwl:hasOBONamespace>GAZ</oboInOwl:hasOBONamespace>
        <oboInOwl:id>GAZ:00030222</oboInOwl:id>
        <rdfs:label>One Tree Hill</rdfs:label>
    </owl:NamedIndividual>
    


    <!-- http://purl.obolibrary.org/obo/GAZ_00030223 -->

    <owl:NamedIndividual rdf:about="http://purl.obolibrary.org/obo/GAZ_00030223">
        <obo:RO_0001025 rdf:resource="http://purl.obolibrary.org/obo/GAZ_00030225"/>
        <obo:IAO_0000115>The smallest, oldest and furthest downstream of the three artificial lakes of the Waitaki hydroelectric project in New Zealand&apos;s South Island. It lies below lakes Aviemore and Benmore on the Waitaki River, close to the town of Kurow. It is part of the traditional boundary of the Canterbury and Otago regions. The lake is created by Waitaki Dam, a 36m high spill weir dam built between 1928 and 1934.</obo:IAO_0000115>
        <oboInOwl:hasOBONamespace>GAZ</oboInOwl:hasOBONamespace>
        <oboInOwl:id>GAZ:00030223</oboInOwl:id>
        <rdfs:label>Lake Waitaki</rdfs:label>
    </owl:NamedIndividual>
    


    <!-- http://purl.obolibrary.org/obo/GAZ_00030224 -->

    <owl:NamedIndividual rdf:about="http://purl.obolibrary.org/obo/GAZ_00030224">
        <obo:RO_0001025 rdf:resource="http://purl.obolibrary.org/obo/GAZ_00030223"/>
        <obo:IAO_0000115>A stream running into Lake Waitaki on its south side.</obo:IAO_0000115>
        <oboInOwl:hasOBONamespace>GAZ</oboInOwl:hasOBONamespace>
        <oboInOwl:id>GAZ:00030224</oboInOwl:id>
        <rdfs:label>Awahokomo Creek</rdfs:label>
    </owl:NamedIndividual>
    


    <!-- http://purl.obolibrary.org/obo/GAZ_00030225 -->

    <owl:NamedIndividual rdf:about="http://purl.obolibrary.org/obo/GAZ_00030225">
        <obo:RO_0001025 rdf:resource="http://purl.obolibrary.org/obo/GAZ_00004764"/>
        <obo:IAO_0000115>A large river in the South Island of New Zealand, some 110 km long. It is the major river of the Mackenzie Basin. It is a braided river which has Lake Benmore, Lake Aviemore and Lake Waitaki at its headwaters. These are ultimately fed by three large glacial lakes, Pukaki, Tekapo, and Ohau. Lake Benmore and Lake Aviemore are contained by hydroelectric dams, Benmore Dam and Aviemore Dam. The Waitaki has several tributaries, notably the Ahuriri River and the Hakataramea River. It passes Kurow and Glenavy before entering the Pacific Ocean between Timaru and Oamaru on the east coast of the South Island.</obo:IAO_0000115>
        <oboInOwl:hasOBONamespace>GAZ</oboInOwl:hasOBONamespace>
        <oboInOwl:id>GAZ:00030225</oboInOwl:id>
        <rdfs:label>Waitaki River</rdfs:label>
    </owl:NamedIndividual>
    


    <!-- http://purl.obolibrary.org/obo/GAZ_00030226 -->

    <owl:NamedIndividual rdf:about="http://purl.obolibrary.org/obo/GAZ_00030226">
        <obo:RO_0001025 rdf:resource="http://purl.obolibrary.org/obo/GAZ_00004765"/>
        <oboInOwl:hasOBONamespace>GAZ</oboInOwl:hasOBONamespace>
        <oboInOwl:id>GAZ:00030226</oboInOwl:id>
        <rdfs:label>Awakino River</rdfs:label>
    </owl:NamedIndividual>
    


    <!-- http://purl.obolibrary.org/obo/GAZ_00030227 -->

    <owl:NamedIndividual rdf:about="http://purl.obolibrary.org/obo/GAZ_00030227">
        <obo:RO_0001025 rdf:resource="http://purl.obolibrary.org/obo/GAZ_00004765"/>
        <oboInOwl:hasOBONamespace>GAZ</oboInOwl:hasOBONamespace>
        <oboInOwl:id>GAZ:00030227</oboInOwl:id>
        <rdfs:label>Saint Mary Range</rdfs:label>
    </owl:NamedIndividual>
    


    <!-- http://purl.obolibrary.org/obo/GAZ_00030228 -->

    <owl:NamedIndividual rdf:about="http://purl.obolibrary.org/obo/GAZ_00030228">
        <obo:RO_0001025 rdf:resource="http://purl.obolibrary.org/obo/GAZ_00010246"/>
        <obo:IAO_0000115>A peninsula located in the Canterbury region on the east coast of the South Island of New Zealand, partly surrounded by the Pacific Ocean, and adjacent to the largest city in the South Island, Christchurch.</obo:IAO_0000115>
        <oboInOwl:hasOBONamespace>GAZ</oboInOwl:hasOBONamespace>
        <oboInOwl:id>GAZ:00030228</oboInOwl:id>
        <rdfs:label>Banks Peninsula</rdfs:label>
    </owl:NamedIndividual>
    


    <!-- http://purl.obolibrary.org/obo/GAZ_00030229 -->

    <owl:NamedIndividual rdf:about="http://purl.obolibrary.org/obo/GAZ_00030229">
        <obo:RO_0001025 rdf:resource="http://purl.obolibrary.org/obo/GAZ_00030228"/>
        <oboInOwl:hasOBONamespace>GAZ</oboInOwl:hasOBONamespace>
        <oboInOwl:id>GAZ:00030229</oboInOwl:id>
        <rdfs:label>Otepatotu Reserve</rdfs:label>
    </owl:NamedIndividual>
    


    <!-- http://purl.obolibrary.org/obo/GAZ_00030230 -->

    <owl:NamedIndividual rdf:about="http://purl.obolibrary.org/obo/GAZ_00030230">
        <obo:RO_0001025 rdf:resource="http://purl.obolibrary.org/obo/GAZ_00007723"/>
        <obo:IAO_0000115>A bay that stretches from the base of the Coromandel Peninsula in the west to Cape Runaway in the east. The region is bound by the Kaimai and Mamaku Ranges in the west and extends inland to the sparsely populated forest lands around Rotorua, Kawerau and Murupara. Several islands are located in the bay, notably Mayor Island/Tuhua, Motiti Island, Whale Island and, most famously, the active volcano of Whakaari/White Island.</obo:IAO_0000115>
        <oboInOwl:hasOBONamespace>GAZ</oboInOwl:hasOBONamespace>
        <oboInOwl:id>GAZ:00030230</oboInOwl:id>
        <rdfs:label>Bay of Plenty</rdfs:label>
    </owl:NamedIndividual>
    


    <!-- http://purl.obolibrary.org/obo/GAZ_00030231 -->

    <owl:NamedIndividual rdf:about="http://purl.obolibrary.org/obo/GAZ_00030231">
        <obo:RO_0001025 rdf:resource="http://purl.obolibrary.org/obo/GAZ_00030235"/>
        <obo:IAO_0000115>An island located off the Bay of Plenty coast of New Zealand&apos;s North Island. It is 21 km northeast of Tauranga and 9.4 km North East of Papamoa.</obo:IAO_0000115>
        <oboInOwl:hasOBONamespace>GAZ</oboInOwl:hasOBONamespace>
        <oboInOwl:id>GAZ:00030231</oboInOwl:id>
        <rdfs:label>Motiti Island</rdfs:label>
    </owl:NamedIndividual>
    


    <!-- http://purl.obolibrary.org/obo/GAZ_00030232 -->

    <owl:NamedIndividual rdf:about="http://purl.obolibrary.org/obo/GAZ_00030232">
        <obo:RO_0001025 rdf:resource="http://purl.obolibrary.org/obo/GAZ_00030235"/>
        <obo:IAO_0000115>An island that forms the summit of a largely submerged Pleistocene dacitic-andesitic complex volcano that lies 11 km offshore from Whakatane in the Bay of Plenty. The island is 15 x 5 km wide and elongated in an east-west direction. The 354 m high central dome complex is flanked by East Dome, which forms the eastern tip of the island and is the oldest of the domes, and Pa Hill lava dome, which forms the NW tip of the island. Acid hot springs, steaming ground, and fumaroles are located primarily between the central cone and East Dome. The central cone and east dome are both older than the roughly 42,000 before present (BP) Rotoehu Tephra, and Pa Hill dome is overlain by the 9000 years BP Rotoma Ash but may be considerably older.</obo:IAO_0000115>
        <oboInOwl:hasOBONamespace>GAZ</oboInOwl:hasOBONamespace>
        <oboInOwl:id>GAZ:00030232</oboInOwl:id>
        <rdfs:label>Whale Island</rdfs:label>
    </owl:NamedIndividual>
    


    <!-- http://purl.obolibrary.org/obo/GAZ_00030233 -->

    <owl:NamedIndividual rdf:about="http://purl.obolibrary.org/obo/GAZ_00030233">
        <obo:RO_0001025 rdf:resource="http://purl.obolibrary.org/obo/GAZ_00030235"/>
        <obo:RO_0001025 rdf:resource="http://purl.obolibrary.org/obo/GAZ_00051945"/>
        <obo:IAO_0000115>An island which is the emergent portion of a 15 km wide compound peralkaline lava shield constructed between about 120,000 and 35,000 years ago. A 3 km wide composite caldera was formed in two or three collapse events, the last of which took place about 6300 years ago, and was accompanied by a plinian eruption that produced tephra deposits up to 70 cm thick on mainland North Island. Post-caldera eruptions generated a series of lava domes and flows emplaced from NNE-trending vents within the caldera that have filled it to depths of at least 180 m.</obo:IAO_0000115>
        <oboInOwl:hasOBONamespace>GAZ</oboInOwl:hasOBONamespace>
        <oboInOwl:id>GAZ:00030233</oboInOwl:id>
        <rdfs:label>Mayor Island</rdfs:label>
    </owl:NamedIndividual>
    


    <!-- http://purl.obolibrary.org/obo/GAZ_00030234 -->

    <owl:NamedIndividual rdf:about="http://purl.obolibrary.org/obo/GAZ_00030234">
        <obo:RO_0001025 rdf:resource="http://purl.obolibrary.org/obo/GAZ_00030235"/>
        <obo:RO_0001025 rdf:resource="http://purl.obolibrary.org/obo/GAZ_00051945"/>
        <obo:IAO_0000115>An active andesite stratovolcano, situated 48 km from the east coast of the North Island of New Zealand, in the Bay of Plenty. The island is the emergent summit of a 16 x 18 km submarine volcano. The 321 m high island consists of two overlapping andesitic-to-dacitic stratovolcanoes; the summit crater appears to be breached to the SE because the shoreline corresponds to the level of several notches in the SE crater wall. Volckner Rocks, four sea stacks that are remnants of a lava dome, lie 5 km NNE of White Island.</obo:IAO_0000115>
        <oboInOwl:hasOBONamespace>GAZ</oboInOwl:hasOBONamespace>
        <oboInOwl:id>GAZ:00030234</oboInOwl:id>
        <rdfs:label>Whakaari Island</rdfs:label>
    </owl:NamedIndividual>
    


    <!-- http://purl.obolibrary.org/obo/GAZ_00030235 -->

    <owl:NamedIndividual rdf:about="http://purl.obolibrary.org/obo/GAZ_00030235">
        <obo:RO_0001025 rdf:resource="http://purl.obolibrary.org/obo/GAZ_00030230"/>
        <oboInOwl:hasOBONamespace>GAZ</oboInOwl:hasOBONamespace>
        <oboInOwl:id>GAZ:00030235</oboInOwl:id>
        <rdfs:label>Olive Islands</rdfs:label>
    </owl:NamedIndividual>
    


    <!-- http://purl.obolibrary.org/obo/GAZ_00044917 -->

    <owl:NamedIndividual rdf:about="http://purl.obolibrary.org/obo/GAZ_00044917">
        <rdf:type rdf:resource="http://purl.obolibrary.org/obo/ENVO_00000222"/>
        <obo:RO_0001025 rdf:resource="http://purl.obolibrary.org/obo/GAZ_00007172"/>
        <obo:IAO_0000115>A volcanic island, the main island of the Antipodes Islands.</obo:IAO_0000115>
        <oboInOwl:hasOBONamespace>GAZ</oboInOwl:hasOBONamespace>
        <oboInOwl:id>GAZ:00044917</oboInOwl:id>
        <rdfs:label>Antipodes Island</rdfs:label>
    </owl:NamedIndividual>
    


    <!-- http://purl.obolibrary.org/obo/GAZ_00044918 -->

    <owl:NamedIndividual rdf:about="http://purl.obolibrary.org/obo/GAZ_00044918">
        <obo:RO_0001025 rdf:resource="http://purl.obolibrary.org/obo/GAZ_00007173"/>
        <obo:IAO_0000115>Rocks to the W of Disappointment Island.</obo:IAO_0000115>
        <oboInOwl:hasOBONamespace>GAZ</oboInOwl:hasOBONamespace>
        <oboInOwl:id>GAZ:00044918</oboInOwl:id>
        <rdfs:label>Pinnacle Rocks</rdfs:label>
    </owl:NamedIndividual>
    


    <!-- http://purl.obolibrary.org/obo/GAZ_00044919 -->

    <owl:NamedIndividual rdf:about="http://purl.obolibrary.org/obo/GAZ_00044919">
        <obo:RO_0001025 rdf:resource="http://purl.obolibrary.org/obo/GAZ_00007173"/>
        <obo:IAO_0000115>One of the Auckland Islands, NE of Tucker Point.</obo:IAO_0000115>
        <oboInOwl:hasOBONamespace>GAZ</oboInOwl:hasOBONamespace>
        <oboInOwl:id>GAZ:00044919</oboInOwl:id>
        <rdfs:label>Ocean Island</rdfs:label>
    </owl:NamedIndividual>
    


    <!-- http://purl.obolibrary.org/obo/GAZ_00044920 -->

    <owl:NamedIndividual rdf:about="http://purl.obolibrary.org/obo/GAZ_00044920">
        <obo:RO_0001025 rdf:resource="http://purl.obolibrary.org/obo/GAZ_00007173"/>
        <obo:IAO_0000115>One of the Auckland Islands, E of Terror Cove.</obo:IAO_0000115>
        <oboInOwl:hasOBONamespace>GAZ</oboInOwl:hasOBONamespace>
        <oboInOwl:id>GAZ:00044920</oboInOwl:id>
        <rdfs:label>Shoe Island</rdfs:label>
    </owl:NamedIndividual>
    


    <!-- http://purl.obolibrary.org/obo/GAZ_00044921 -->

    <owl:NamedIndividual rdf:about="http://purl.obolibrary.org/obo/GAZ_00044921">
        <obo:RO_0001025 rdf:resource="http://purl.obolibrary.org/obo/GAZ_00007173"/>
        <obo:IAO_0000115>Rocks off the SE of Adams Island, NW of Astrolable Point.</obo:IAO_0000115>
        <oboInOwl:hasOBONamespace>GAZ</oboInOwl:hasOBONamespace>
        <oboInOwl:id>GAZ:00044921</oboInOwl:id>
        <rdfs:label>Lantern Rocks</rdfs:label>
    </owl:NamedIndividual>
    


    <!-- http://purl.obolibrary.org/obo/GAZ_00044922 -->

    <owl:NamedIndividual rdf:about="http://purl.obolibrary.org/obo/GAZ_00044922">
        <obo:RO_0001025 rdf:resource="http://purl.obolibrary.org/obo/GAZ_00007173"/>
        <oboInOwl:hasOBONamespace>GAZ</oboInOwl:hasOBONamespace>
        <oboInOwl:id>GAZ:00044922</oboInOwl:id>
        <rdfs:label>Invercauld Rock</rdfs:label>
    </owl:NamedIndividual>
    


    <!-- http://purl.obolibrary.org/obo/GAZ_00044923 -->

    <owl:NamedIndividual rdf:about="http://purl.obolibrary.org/obo/GAZ_00044923">
        <obo:RO_0001025 rdf:resource="http://purl.obolibrary.org/obo/GAZ_00007173"/>
        <obo:IAO_0000115>One of the Auckland Islands, between Auckland Island and Enderby Island.</obo:IAO_0000115>
        <oboInOwl:hasOBONamespace>GAZ</oboInOwl:hasOBONamespace>
        <oboInOwl:id>GAZ:00044923</oboInOwl:id>
        <rdfs:label>Rose Island</rdfs:label>
    </owl:NamedIndividual>
    


    <!-- http://purl.obolibrary.org/obo/GAZ_00044924 -->

    <owl:NamedIndividual rdf:about="http://purl.obolibrary.org/obo/GAZ_00044924">
        <obo:RO_0001025 rdf:resource="http://purl.obolibrary.org/obo/GAZ_00007173"/>
        <obo:IAO_0000115>One of the Auckland Islands, in Victoria Passage.</obo:IAO_0000115>
        <oboInOwl:hasOBONamespace>GAZ</oboInOwl:hasOBONamespace>
        <oboInOwl:id>GAZ:00044924</oboInOwl:id>
        <rdfs:label>Monumental Island</rdfs:label>
    </owl:NamedIndividual>
    


    <!-- http://purl.obolibrary.org/obo/GAZ_00044925 -->

    <owl:NamedIndividual rdf:about="http://purl.obolibrary.org/obo/GAZ_00044925">
        <obo:RO_0001025 rdf:resource="http://purl.obolibrary.org/obo/GAZ_00007173"/>
        <obo:IAO_0000115>One of the Auckland Islands, in Carnley Harbour, N of Anjou Point.</obo:IAO_0000115>
        <oboInOwl:hasOBONamespace>GAZ</oboInOwl:hasOBONamespace>
        <oboInOwl:id>GAZ:00044925</oboInOwl:id>
        <rdfs:label>Masked Island</rdfs:label>
    </owl:NamedIndividual>
    


    <!-- http://purl.obolibrary.org/obo/GAZ_00044926 -->

    <owl:NamedIndividual rdf:about="http://purl.obolibrary.org/obo/GAZ_00044926">
        <obo:RO_0001025 rdf:resource="http://purl.obolibrary.org/obo/GAZ_00007173"/>
        <obo:IAO_0000115>Rocks to the E of Disappointment Island.</obo:IAO_0000115>
        <oboInOwl:hasOBONamespace>GAZ</oboInOwl:hasOBONamespace>
        <oboInOwl:id>GAZ:00044926</oboInOwl:id>
        <rdfs:label>Sugar Loaf Rocks</rdfs:label>
    </owl:NamedIndividual>
    


    <!-- http://purl.obolibrary.org/obo/GAZ_00044927 -->

    <owl:NamedIndividual rdf:about="http://purl.obolibrary.org/obo/GAZ_00044927">
        <obo:RO_0001025 rdf:resource="http://purl.obolibrary.org/obo/GAZ_00007173"/>
        <obo:IAO_0000115>Rocks to the E of Disappointment Island.</obo:IAO_0000115>
        <oboInOwl:hasOBONamespace>GAZ</oboInOwl:hasOBONamespace>
        <oboInOwl:id>GAZ:00044927</oboInOwl:id>
        <rdfs:label>Shag Rock</rdfs:label>
    </owl:NamedIndividual>
    


    <!-- http://purl.obolibrary.org/obo/GAZ_00044928 -->

    <owl:NamedIndividual rdf:about="http://purl.obolibrary.org/obo/GAZ_00044928">
        <obo:RO_0001025 rdf:resource="http://purl.obolibrary.org/obo/GAZ_00007173"/>
        <obo:IAO_0000115>A rock off the NW coast of Auckland Island, W of Rose Island.</obo:IAO_0000115>
        <oboInOwl:hasOBONamespace>GAZ</oboInOwl:hasOBONamespace>
        <oboInOwl:id>GAZ:00044928</oboInOwl:id>
        <rdfs:label>Pillar Rock</rdfs:label>
    </owl:NamedIndividual>
    


    <!-- http://purl.obolibrary.org/obo/GAZ_00044929 -->

    <owl:NamedIndividual rdf:about="http://purl.obolibrary.org/obo/GAZ_00044929">
        <obo:RO_0001025 rdf:resource="http://purl.obolibrary.org/obo/GAZ_00007173"/>
        <obo:IAO_0000115>One of the Auckland Islands, SE of Yule Island.</obo:IAO_0000115>
        <oboInOwl:hasOBONamespace>GAZ</oboInOwl:hasOBONamespace>
        <oboInOwl:id>GAZ:00044929</oboInOwl:id>
        <rdfs:label>Yule Island</rdfs:label>
    </owl:NamedIndividual>
    


    <!-- http://purl.obolibrary.org/obo/GAZ_00044930 -->

    <owl:NamedIndividual rdf:about="http://purl.obolibrary.org/obo/GAZ_00044930">
        <obo:RO_0001025 rdf:resource="http://purl.obolibrary.org/obo/GAZ_00007173"/>
        <obo:IAO_0000115>One of the Auckland Islands, in the North Arm.</obo:IAO_0000115>
        <oboInOwl:hasOBONamespace>GAZ</oboInOwl:hasOBONamespace>
        <oboInOwl:id>GAZ:00044930</oboInOwl:id>
        <rdfs:label>Figure of Eight Island</rdfs:label>
    </owl:NamedIndividual>
    


    <!-- http://purl.obolibrary.org/obo/GAZ_00044931 -->

    <owl:NamedIndividual rdf:about="http://purl.obolibrary.org/obo/GAZ_00044931">
        <obo:RO_0001025 rdf:resource="http://purl.obolibrary.org/obo/GAZ_00007173"/>
        <obo:IAO_0000115>One of the Auckland Islands, between Lindley Point and SW of Rose Island.</obo:IAO_0000115>
        <oboInOwl:hasOBONamespace>GAZ</oboInOwl:hasOBONamespace>
        <oboInOwl:id>GAZ:00044931</oboInOwl:id>
        <rdfs:label>Friday Island</rdfs:label>
    </owl:NamedIndividual>
    


    <!-- http://purl.obolibrary.org/obo/GAZ_00044932 -->

    <owl:NamedIndividual rdf:about="http://purl.obolibrary.org/obo/GAZ_00044932">
        <obo:RO_0001025 rdf:resource="http://purl.obolibrary.org/obo/GAZ_00007173"/>
        <obo:IAO_0000115>One of the Auckland Islands, NE of Crozier Point.</obo:IAO_0000115>
        <oboInOwl:hasOBONamespace>GAZ</oboInOwl:hasOBONamespace>
        <oboInOwl:id>GAZ:00044932</oboInOwl:id>
        <rdfs:label>Frenchs Island</rdfs:label>
    </owl:NamedIndividual>
    


    <!-- http://purl.obolibrary.org/obo/GAZ_00044933 -->

    <owl:NamedIndividual rdf:about="http://purl.obolibrary.org/obo/GAZ_00044933">
        <obo:RO_0001025 rdf:resource="http://purl.obolibrary.org/obo/GAZ_00007173"/>
        <obo:IAO_0000115>One of the Auckland Islands.</obo:IAO_0000115>
        <oboInOwl:hasOBONamespace>GAZ</oboInOwl:hasOBONamespace>
        <oboInOwl:id>GAZ:00044933</oboInOwl:id>
        <rdfs:label>Fabulous Island</rdfs:label>
    </owl:NamedIndividual>
    


    <!-- http://purl.obolibrary.org/obo/GAZ_00044934 -->

    <owl:NamedIndividual rdf:about="http://purl.obolibrary.org/obo/GAZ_00044934">
        <obo:RO_0001025 rdf:resource="http://purl.obolibrary.org/obo/GAZ_00007173"/>
        <obo:IAO_0000115>Rocks off the NW coast of Auckland Island.</obo:IAO_0000115>
        <oboInOwl:hasOBONamespace>GAZ</oboInOwl:hasOBONamespace>
        <oboInOwl:id>GAZ:00044934</oboInOwl:id>
        <rdfs:label>Five Sisters Rocks</rdfs:label>
    </owl:NamedIndividual>
    


    <!-- http://purl.obolibrary.org/obo/GAZ_00044935 -->

    <owl:NamedIndividual rdf:about="http://purl.obolibrary.org/obo/GAZ_00044935">
        <obo:RO_0001025 rdf:resource="http://purl.obolibrary.org/obo/GAZ_00007173"/>
        <oboInOwl:hasOBONamespace>GAZ</oboInOwl:hasOBONamespace>
        <oboInOwl:id>GAZ:00044935</oboInOwl:id>
        <rdfs:label>Chapel Rock</rdfs:label>
    </owl:NamedIndividual>
    


    <!-- http://purl.obolibrary.org/obo/GAZ_00044936 -->

    <owl:NamedIndividual rdf:about="http://purl.obolibrary.org/obo/GAZ_00044936">
        <obo:RO_0001025 rdf:resource="http://purl.obolibrary.org/obo/GAZ_00007173"/>
        <obo:IAO_0000115>A rock SE of Black Head.</obo:IAO_0000115>
        <oboInOwl:hasOBONamespace>GAZ</oboInOwl:hasOBONamespace>
        <oboInOwl:id>GAZ:00044936</oboInOwl:id>
        <rdfs:label>Beacon Rock</rdfs:label>
    </owl:NamedIndividual>
    


    <!-- http://purl.obolibrary.org/obo/GAZ_00044937 -->

    <owl:NamedIndividual rdf:about="http://purl.obolibrary.org/obo/GAZ_00044937">
        <obo:RO_0001025 rdf:resource="http://purl.obolibrary.org/obo/GAZ_00007173"/>
        <obo:IAO_0000115>One of the Auckland Islands, N of Beacon Point.</obo:IAO_0000115>
        <oboInOwl:hasOBONamespace>GAZ</oboInOwl:hasOBONamespace>
        <oboInOwl:id>GAZ:00044937</oboInOwl:id>
        <rdfs:label>Davis Island</rdfs:label>
    </owl:NamedIndividual>
    


    <!-- http://purl.obolibrary.org/obo/GAZ_00044938 -->

    <owl:NamedIndividual rdf:about="http://purl.obolibrary.org/obo/GAZ_00044938">
        <obo:RO_0001025 rdf:resource="http://purl.obolibrary.org/obo/GAZ_00007173"/>
        <obo:IAO_0000115>Rocks to the SW of Black Head.</obo:IAO_0000115>
        <oboInOwl:hasOBONamespace>GAZ</oboInOwl:hasOBONamespace>
        <oboInOwl:id>GAZ:00044938</oboInOwl:id>
        <rdfs:label>Compadre Rock</rdfs:label>
    </owl:NamedIndividual>
    


    <!-- http://purl.obolibrary.org/obo/GAZ_00044939 -->

    <owl:NamedIndividual rdf:about="http://purl.obolibrary.org/obo/GAZ_00044939">
        <obo:RO_0001025 rdf:resource="http://purl.obolibrary.org/obo/GAZ_00007173"/>
        <obo:IAO_0000115>Rocks to the E of Aukland Island.</obo:IAO_0000115>
        <oboInOwl:hasOBONamespace>GAZ</oboInOwl:hasOBONamespace>
        <oboInOwl:id>GAZ:00044939</oboInOwl:id>
        <rdfs:label>Blanche Rock</rdfs:label>
    </owl:NamedIndividual>
    


    <!-- http://purl.obolibrary.org/obo/GAZ_00044940 -->

    <owl:NamedIndividual rdf:about="http://purl.obolibrary.org/obo/GAZ_00044940">
        <obo:RO_0001025 rdf:resource="http://purl.obolibrary.org/obo/GAZ_00007173"/>
        <obo:IAO_0000115>Rocks to the immediate W of Northwest Cape.</obo:IAO_0000115>
        <oboInOwl:hasOBONamespace>GAZ</oboInOwl:hasOBONamespace>
        <oboInOwl:id>GAZ:00044940</oboInOwl:id>
        <rdfs:label>Column Rocks</rdfs:label>
    </owl:NamedIndividual>
    


    <!-- http://purl.obolibrary.org/obo/GAZ_00044941 -->

    <owl:NamedIndividual rdf:about="http://purl.obolibrary.org/obo/GAZ_00044941">
        <obo:RO_0001025 rdf:resource="http://purl.obolibrary.org/obo/GAZ_00007173"/>
        <obo:IAO_0000115>Rocks to the NW of Embrasure Point, Adams Island.</obo:IAO_0000115>
        <oboInOwl:hasOBONamespace>GAZ</oboInOwl:hasOBONamespace>
        <oboInOwl:id>GAZ:00044941</oboInOwl:id>
        <rdfs:label>Adams Rocks</rdfs:label>
    </owl:NamedIndividual>
    


    <!-- http://purl.obolibrary.org/obo/GAZ_00044942 -->

    <owl:NamedIndividual rdf:about="http://purl.obolibrary.org/obo/GAZ_00044942">
        <obo:RO_0001025 rdf:resource="http://purl.obolibrary.org/obo/GAZ_00007173"/>
        <obo:IAO_0000115>A small rock N of Cape Bennett.</obo:IAO_0000115>
        <oboInOwl:hasOBONamespace>GAZ</oboInOwl:hasOBONamespace>
        <oboInOwl:id>GAZ:00044942</oboInOwl:id>
        <rdfs:label>Archer Rock</rdfs:label>
    </owl:NamedIndividual>
    


    <!-- http://purl.obolibrary.org/obo/GAZ_00044943 -->

    <owl:NamedIndividual rdf:about="http://purl.obolibrary.org/obo/GAZ_00044943">
        <obo:RO_0001025 rdf:resource="http://purl.obolibrary.org/obo/GAZ_00007173"/>
        <obo:IAO_0000115>Small rocks off the S coast of Adams Islands.</obo:IAO_0000115>
        <oboInOwl:hasOBONamespace>GAZ</oboInOwl:hasOBONamespace>
        <oboInOwl:id>GAZ:00044943</oboInOwl:id>
        <rdfs:label>Amherst Rock</rdfs:label>
    </owl:NamedIndividual>
    


    <!-- http://purl.obolibrary.org/obo/GAZ_00044989 -->

    <owl:NamedIndividual rdf:about="http://purl.obolibrary.org/obo/GAZ_00044989">
        <obo:RO_0001025 rdf:resource="http://purl.obolibrary.org/obo/GAZ_00007176"/>
        <obo:IAO_0000115>A group of islets; a part of the Snares Island group. They lie some 5 km to the WSW off the main island North East Island, which lies approximately 200 km south of New Zealand&apos;s South Island. The Western Chain island is some 2 km long in NW direction, and the highest elevation of 44 m is at the southernmost Island.</obo:IAO_0000115>
        <oboInOwl:hasOBONamespace>GAZ</oboInOwl:hasOBONamespace>
        <oboInOwl:id>GAZ:00044989</oboInOwl:id>
        <rdfs:label>Western Chain Islands</rdfs:label>
    </owl:NamedIndividual>
    


    <!-- http://purl.obolibrary.org/obo/GAZ_00044990 -->

    <owl:NamedIndividual rdf:about="http://purl.obolibrary.org/obo/GAZ_00044990">
        <obo:RO_0001025 rdf:resource="http://purl.obolibrary.org/obo/GAZ_00007176"/>
        <obo:IAO_0000115>The second largest island of the Snares Island group just off the South Promontory of the main island North East Island, which lies approximately 200 km south of New Zealand&apos;s South Island. The island is some 1 by 0.5 km long in SW direction, and the highest elevation is 86 m.</obo:IAO_0000115>
        <oboInOwl:hasOBONamespace>GAZ</oboInOwl:hasOBONamespace>
        <oboInOwl:id>GAZ:00044990</oboInOwl:id>
        <rdfs:label>Broughton Island</rdfs:label>
    </owl:NamedIndividual>
    


    <!-- http://purl.obolibrary.org/obo/GAZ_00044991 -->

    <owl:NamedIndividual rdf:about="http://purl.obolibrary.org/obo/GAZ_00044991">
        <obo:RO_0001025 rdf:resource="http://purl.obolibrary.org/obo/GAZ_00007176"/>
        <obo:IAO_0000115>The main island of the Snares Island group. The island forms a central triangle with peninsulas to the north, south and to the west and is some 3 by 2.5 km wide. Off the South Promontory lies Broughton Island, the second largest island in the group. South off the western peninsula coast lies the islet Alert Stack and off the North Promontory lies the North and South Daption Rocks.</obo:IAO_0000115>
        <oboInOwl:hasOBONamespace>GAZ</oboInOwl:hasOBONamespace>
        <oboInOwl:id>GAZ:00044991</oboInOwl:id>
        <rdfs:label>North East Island</rdfs:label>
    </owl:NamedIndividual>
    


    <!-- http://purl.obolibrary.org/obo/GAZ_00044992 -->

    <owl:NamedIndividual rdf:about="http://purl.obolibrary.org/obo/GAZ_00044992">
        <obo:RO_0001025 rdf:resource="http://purl.obolibrary.org/obo/GAZ_00044989"/>
        <obo:IAO_0000115>One of the Western Chain Islands.</obo:IAO_0000115>
        <oboInOwl:hasOBONamespace>GAZ</oboInOwl:hasOBONamespace>
        <oboInOwl:id>GAZ:00044992</oboInOwl:id>
        <rdfs:label>Rua Island</rdfs:label>
    </owl:NamedIndividual>
    


    <!-- http://purl.obolibrary.org/obo/GAZ_00044993 -->

    <owl:NamedIndividual rdf:about="http://purl.obolibrary.org/obo/GAZ_00044993">
        <obo:RO_0001025 rdf:resource="http://purl.obolibrary.org/obo/GAZ_00044989"/>
        <obo:IAO_0000115>One of the Western Chain Islands.</obo:IAO_0000115>
        <oboInOwl:hasOBONamespace>GAZ</oboInOwl:hasOBONamespace>
        <oboInOwl:id>GAZ:00044993</oboInOwl:id>
        <rdfs:label>Rua Island</rdfs:label>
    </owl:NamedIndividual>
    


    <!-- http://purl.obolibrary.org/obo/GAZ_00044994 -->

    <owl:NamedIndividual rdf:about="http://purl.obolibrary.org/obo/GAZ_00044994">
        <obo:RO_0001025 rdf:resource="http://purl.obolibrary.org/obo/GAZ_00044989"/>
        <obo:IAO_0000115>One of the Western Chain Islands.</obo:IAO_0000115>
        <oboInOwl:hasOBONamespace>GAZ</oboInOwl:hasOBONamespace>
        <oboInOwl:id>GAZ:00044994</oboInOwl:id>
        <rdfs:label>Rima Island</rdfs:label>
    </owl:NamedIndividual>
    


    <!-- http://purl.obolibrary.org/obo/GAZ_00044995 -->

    <owl:NamedIndividual rdf:about="http://purl.obolibrary.org/obo/GAZ_00044995">
        <obo:RO_0001025 rdf:resource="http://purl.obolibrary.org/obo/GAZ_00044989"/>
        <obo:IAO_0000115>One of the Western Chain Islands.</obo:IAO_0000115>
        <oboInOwl:hasOBONamespace>GAZ</oboInOwl:hasOBONamespace>
        <oboInOwl:id>GAZ:00044995</oboInOwl:id>
        <rdfs:label>Wha Island</rdfs:label>
    </owl:NamedIndividual>
    


    <!-- http://purl.obolibrary.org/obo/GAZ_00044996 -->

    <owl:NamedIndividual rdf:about="http://purl.obolibrary.org/obo/GAZ_00044996">
        <obo:RO_0001025 rdf:resource="http://purl.obolibrary.org/obo/GAZ_00044989"/>
        <obo:IAO_0000115>One of the Western Chain Islands.</obo:IAO_0000115>
        <oboInOwl:hasOBONamespace>GAZ</oboInOwl:hasOBONamespace>
        <oboInOwl:id>GAZ:00044996</oboInOwl:id>
        <rdfs:label>Toru Island</rdfs:label>
    </owl:NamedIndividual>
    


    <!-- http://purl.obolibrary.org/obo/GAZ_00046912 -->

    <owl:NamedIndividual rdf:about="http://purl.obolibrary.org/obo/GAZ_00046912">
        <obo:RO_0001025 rdf:resource="http://purl.obolibrary.org/obo/GAZ_00004781"/>
        <obo:RO_0001025 rdf:resource="http://purl.obolibrary.org/obo/GAZ_00030230"/>
        <obo:IAO_0000115>A small group of rocky islets to the southeast of Mercury Bay in the North Island of New Zealand. They are located off the coast of the Coromandel Peninsula, 20 km east of the mouth of the Tairua River.</obo:IAO_0000115>
        <oboInOwl:hasOBONamespace>GAZ</oboInOwl:hasOBONamespace>
        <oboInOwl:id>GAZ:00046912</oboInOwl:id>
        <rdfs:label>Alderman Islands</rdfs:label>
    </owl:NamedIndividual>
    


    <!-- http://purl.obolibrary.org/obo/GAZ_00046913 -->

    <owl:NamedIndividual rdf:about="http://purl.obolibrary.org/obo/GAZ_00046913">
        <obo:RO_0001025 rdf:resource="http://purl.obolibrary.org/obo/GAZ_00046912"/>
        <obo:IAO_0000115>One of the Alderman Islands.</obo:IAO_0000115>
        <oboInOwl:hasOBONamespace>GAZ</oboInOwl:hasOBONamespace>
        <oboInOwl:id>GAZ:00046913</oboInOwl:id>
        <rdfs:label>Hongiora Island</rdfs:label>
    </owl:NamedIndividual>
    


    <!-- http://purl.obolibrary.org/obo/GAZ_00046914 -->

    <owl:NamedIndividual rdf:about="http://purl.obolibrary.org/obo/GAZ_00046914">
        <obo:RO_0001025 rdf:resource="http://purl.obolibrary.org/obo/GAZ_00046912"/>
        <obo:IAO_0000115>One of the Alderman Islands.</obo:IAO_0000115>
        <oboInOwl:hasOBONamespace>GAZ</oboInOwl:hasOBONamespace>
        <oboInOwl:id>GAZ:00046914</oboInOwl:id>
        <rdfs:label>Middle Island</rdfs:label>
    </owl:NamedIndividual>
    


    <!-- http://purl.obolibrary.org/obo/GAZ_00046915 -->

    <owl:NamedIndividual rdf:about="http://purl.obolibrary.org/obo/GAZ_00046915">
        <obo:RO_0001025 rdf:resource="http://purl.obolibrary.org/obo/GAZ_00046912"/>
        <obo:IAO_0000115>One of the Alderman Islands.</obo:IAO_0000115>
        <oboInOwl:hasOBONamespace>GAZ</oboInOwl:hasOBONamespace>
        <oboInOwl:id>GAZ:00046915</oboInOwl:id>
        <rdfs:label>Ruamahuanui Island</rdfs:label>
    </owl:NamedIndividual>
    


    <!-- http://purl.obolibrary.org/obo/GAZ_00046916 -->

    <owl:NamedIndividual rdf:about="http://purl.obolibrary.org/obo/GAZ_00046916">
        <obo:RO_0001025 rdf:resource="http://purl.obolibrary.org/obo/GAZ_00046912"/>
        <obo:IAO_0000115>One of the Alderman Islands.</obo:IAO_0000115>
        <oboInOwl:hasOBONamespace>GAZ</oboInOwl:hasOBONamespace>
        <oboInOwl:id>GAZ:00046916</oboInOwl:id>
        <rdfs:label>Ruamahuaiti Island</rdfs:label>
    </owl:NamedIndividual>
    


    <!-- http://purl.obolibrary.org/obo/GAZ_00046917 -->

    <owl:NamedIndividual rdf:about="http://purl.obolibrary.org/obo/GAZ_00046917">
        <obo:RO_0001025 rdf:resource="http://purl.obolibrary.org/obo/GAZ_00047047"/>
        <obo:IAO_0000115>A fjord on the south west corner of New Zealand, in Fiordland National Park.</obo:IAO_0000115>
        <oboInOwl:hasOBONamespace>GAZ</oboInOwl:hasOBONamespace>
        <oboInOwl:id>GAZ:00046917</oboInOwl:id>
        <rdfs:label>Dusky Sound</rdfs:label>
    </owl:NamedIndividual>
    


    <!-- http://purl.obolibrary.org/obo/GAZ_00046918 -->

    <owl:NamedIndividual rdf:about="http://purl.obolibrary.org/obo/GAZ_00046918">
        <obo:RO_0001025 rdf:resource="http://purl.obolibrary.org/obo/GAZ_00046917"/>
        <obo:IAO_0000115>An island in Dusky Sound, Fiordland National Park in the Southland district of New Zealand.</obo:IAO_0000115>
        <oboInOwl:hasOBONamespace>GAZ</oboInOwl:hasOBONamespace>
        <oboInOwl:id>GAZ:00046918</oboInOwl:id>
        <rdfs:label>Anchor Island</rdfs:label>
    </owl:NamedIndividual>
    


    <!-- http://purl.obolibrary.org/obo/GAZ_00046919 -->

    <owl:NamedIndividual rdf:about="http://purl.obolibrary.org/obo/GAZ_00046919">
        <obo:RO_0001025 rdf:resource="http://purl.obolibrary.org/obo/GAZ_00046917"/>
        <obo:IAO_0000115>An island in Dusky Sound.</obo:IAO_0000115>
        <oboInOwl:hasOBONamespace>GAZ</oboInOwl:hasOBONamespace>
        <oboInOwl:id>GAZ:00046919</oboInOwl:id>
        <rdfs:label>Long Island</rdfs:label>
    </owl:NamedIndividual>
    


    <!-- http://purl.obolibrary.org/obo/GAZ_00046920 -->

    <owl:NamedIndividual rdf:about="http://purl.obolibrary.org/obo/GAZ_00046920">
        <obo:RO_0001025 rdf:resource="http://purl.obolibrary.org/obo/GAZ_00046917"/>
        <obo:IAO_0000115>An island in Dusky Sound.</obo:IAO_0000115>
        <oboInOwl:hasOBONamespace>GAZ</oboInOwl:hasOBONamespace>
        <oboInOwl:id>GAZ:00046920</oboInOwl:id>
        <rdfs:label>Cooper Island</rdfs:label>
    </owl:NamedIndividual>
    


    <!-- http://purl.obolibrary.org/obo/GAZ_00046921 -->

    <owl:NamedIndividual rdf:about="http://purl.obolibrary.org/obo/GAZ_00046921">
        <obo:RO_0001025 rdf:resource="http://purl.obolibrary.org/obo/GAZ_00047047"/>
        <obo:IAO_0000115>An island in Fiordland, in the southwest of New Zealand. Resolution Island is separated from the mainland of the South Island by Dusky Sound and Breaksea Sound.</obo:IAO_0000115>
        <oboInOwl:hasOBONamespace>GAZ</oboInOwl:hasOBONamespace>
        <oboInOwl:id>GAZ:00046921</oboInOwl:id>
        <rdfs:label>Resolution Island</rdfs:label>
    </owl:NamedIndividual>
    


    <!-- http://purl.obolibrary.org/obo/GAZ_00046922 -->

    <owl:NamedIndividual rdf:about="http://purl.obolibrary.org/obo/GAZ_00046922">
        <obo:RO_0001025 rdf:resource="http://purl.obolibrary.org/obo/GAZ_00008572"/>
        <obo:IAO_0000115>A tiny island located off the southwest coast of Stewart Island, New Zealand and part of Rakiura National Park.</obo:IAO_0000115>
        <oboInOwl:hasOBONamespace>GAZ</oboInOwl:hasOBONamespace>
        <oboInOwl:id>GAZ:00046922</oboInOwl:id>
        <rdfs:label>Anchorage Island</rdfs:label>
    </owl:NamedIndividual>
    


    <!-- http://purl.obolibrary.org/obo/GAZ_00046923 -->

    <owl:NamedIndividual rdf:about="http://purl.obolibrary.org/obo/GAZ_00046923">
        <obo:RO_0001025 rdf:resource="http://purl.obolibrary.org/obo/GAZ_00008569"/>
        <obo:IAO_0000115>A small island in the Northland Region of New Zealand. It lies off Taiharuru Head, directly east of Whangarei.</obo:IAO_0000115>
        <oboInOwl:hasOBONamespace>GAZ</oboInOwl:hasOBONamespace>
        <oboInOwl:id>GAZ:00046923</oboInOwl:id>
        <rdfs:label>Arakaninihi Island</rdfs:label>
    </owl:NamedIndividual>
    


    <!-- http://purl.obolibrary.org/obo/GAZ_00046924 -->

    <owl:NamedIndividual rdf:about="http://purl.obolibrary.org/obo/GAZ_00046924">
        <obo:RO_0001025 rdf:resource="http://purl.obolibrary.org/obo/GAZ_00008569"/>
        <obo:IAO_0000115>An island in the Northland Region of New Zealand.</obo:IAO_0000115>
        <oboInOwl:hasOBONamespace>GAZ</oboInOwl:hasOBONamespace>
        <oboInOwl:id>GAZ:00046924</oboInOwl:id>
        <rdfs:label>Araara Island</rdfs:label>
    </owl:NamedIndividual>
    


    <!-- http://purl.obolibrary.org/obo/GAZ_00046925 -->

    <owl:NamedIndividual rdf:about="http://purl.obolibrary.org/obo/GAZ_00046925">
        <obo:RO_0001025 rdf:resource="http://purl.obolibrary.org/obo/GAZ_00000469"/>
        <obo:IAO_0000115>An extensive network of sea-drowned valleys (created by a combination of land subsidence and rising sea levels at the north of the South Island of New Zealand. They lie between Tasman Bay in the west and Cloudy Bay in the south-east.</obo:IAO_0000115>
        <oboInOwl:hasOBONamespace>GAZ</oboInOwl:hasOBONamespace>
        <oboInOwl:id>GAZ:00046925</oboInOwl:id>
        <rdfs:label>Marlborough Sounds</rdfs:label>
    </owl:NamedIndividual>
    


    <!-- http://purl.obolibrary.org/obo/GAZ_00046926 -->

    <owl:NamedIndividual rdf:about="http://purl.obolibrary.org/obo/GAZ_00046926">
        <obo:RO_0001025 rdf:resource="http://purl.obolibrary.org/obo/GAZ_00000469"/>
        <obo:RO_0001025 rdf:resource="http://purl.obolibrary.org/obo/GAZ_00008569"/>
        <obo:IAO_0000115>A small island at Kerikeri in the Northland Region of New Zealand, owned and managed by the Queen Elizabeth II National Trust.</obo:IAO_0000115>
        <oboInOwl:hasOBONamespace>GAZ</oboInOwl:hasOBONamespace>
        <oboInOwl:id>GAZ:00046926</oboInOwl:id>
        <rdfs:label>Aroha Island</rdfs:label>
    </owl:NamedIndividual>
    


    <!-- http://purl.obolibrary.org/obo/GAZ_00046929 -->

    <owl:NamedIndividual rdf:about="http://purl.obolibrary.org/obo/GAZ_00046929">
        <obo:RO_0001025 rdf:resource="http://purl.obolibrary.org/obo/GAZ_00000469"/>
        <obo:IAO_0000115>A strait between the North and South Islands of New Zealand. Twenty km wide at its narrowest point, its north side stands the city of Wellington; on the south side lie the Marlborough Sounds and Cloudy Bay.</obo:IAO_0000115>
        <oboInOwl:hasOBONamespace>GAZ</oboInOwl:hasOBONamespace>
        <oboInOwl:id>GAZ:00046929</oboInOwl:id>
        <rdfs:label>Cook Strait</rdfs:label>
    </owl:NamedIndividual>
    


    <!-- http://purl.obolibrary.org/obo/GAZ_00046930 -->

    <owl:NamedIndividual rdf:about="http://purl.obolibrary.org/obo/GAZ_00046930">
        <obo:RO_0001025 rdf:resource="http://purl.obolibrary.org/obo/GAZ_00046929"/>
        <oboInOwl:hasOBONamespace>GAZ</oboInOwl:hasOBONamespace>
        <oboInOwl:id>GAZ:00046930</oboInOwl:id>
        <rdfs:label>The Brothers</rdfs:label>
    </owl:NamedIndividual>
    


    <!-- http://purl.obolibrary.org/obo/GAZ_00046931 -->

    <owl:NamedIndividual rdf:about="http://purl.obolibrary.org/obo/GAZ_00046931">
        <obo:RO_0001025 rdf:resource="http://purl.obolibrary.org/obo/GAZ_00046930"/>
        <oboInOwl:hasOBONamespace>GAZ</oboInOwl:hasOBONamespace>
        <oboInOwl:id>GAZ:00046931</oboInOwl:id>
        <rdfs:label>North Brother island</rdfs:label>
    </owl:NamedIndividual>
    


    <!-- http://purl.obolibrary.org/obo/GAZ_00046932 -->

    <owl:NamedIndividual rdf:about="http://purl.obolibrary.org/obo/GAZ_00046932">
        <obo:RO_0001025 rdf:resource="http://purl.obolibrary.org/obo/GAZ_00008569"/>
        <obo:IAO_0000115>A small group of islands in Whangaroa on Northland&apos;s East Coast in northern New Zealand. They lie five km to the east of Matauri Bay on the mainland.</obo:IAO_0000115>
        <oboInOwl:hasOBONamespace>GAZ</oboInOwl:hasOBONamespace>
        <oboInOwl:id>GAZ:00046932</oboInOwl:id>
        <rdfs:label>Cavalli Islands</rdfs:label>
    </owl:NamedIndividual>
    


    <!-- http://purl.obolibrary.org/obo/GAZ_00046933 -->

    <owl:NamedIndividual rdf:about="http://purl.obolibrary.org/obo/GAZ_00046933">
        <obo:RO_0001025 rdf:resource="http://purl.obolibrary.org/obo/GAZ_00046932"/>
        <obo:IAO_0000115>One of the Cavalli Islands.</obo:IAO_0000115>
        <oboInOwl:hasOBONamespace>GAZ</oboInOwl:hasOBONamespace>
        <oboInOwl:id>GAZ:00046933</oboInOwl:id>
        <rdfs:label>Motutapere Island</rdfs:label>
    </owl:NamedIndividual>
    


    <!-- http://purl.obolibrary.org/obo/GAZ_00046934 -->

    <owl:NamedIndividual rdf:about="http://purl.obolibrary.org/obo/GAZ_00046934">
        <obo:RO_0001025 rdf:resource="http://purl.obolibrary.org/obo/GAZ_00046932"/>
        <obo:IAO_0000115>One of the Cavalli Islands.</obo:IAO_0000115>
        <oboInOwl:hasOBONamespace>GAZ</oboInOwl:hasOBONamespace>
        <oboInOwl:id>GAZ:00046934</oboInOwl:id>
        <rdfs:label>Motukawaiti Island</rdfs:label>
    </owl:NamedIndividual>
    


    <!-- http://purl.obolibrary.org/obo/GAZ_00046935 -->

    <owl:NamedIndividual rdf:about="http://purl.obolibrary.org/obo/GAZ_00046935">
        <obo:RO_0001025 rdf:resource="http://purl.obolibrary.org/obo/GAZ_00046932"/>
        <obo:IAO_0000115>One of the Cavalli Islands.</obo:IAO_0000115>
        <oboInOwl:hasOBONamespace>GAZ</oboInOwl:hasOBONamespace>
        <oboInOwl:id>GAZ:00046935</oboInOwl:id>
        <rdfs:label>Motukawanui Island</rdfs:label>
    </owl:NamedIndividual>
    


    <!-- http://purl.obolibrary.org/obo/GAZ_00046936 -->

    <owl:NamedIndividual rdf:about="http://purl.obolibrary.org/obo/GAZ_00046936">
        <obo:RO_0001025 rdf:resource="http://purl.obolibrary.org/obo/GAZ_00046932"/>
        <obo:IAO_0000115>One of the Cavalli Islands.</obo:IAO_0000115>
        <oboInOwl:hasOBONamespace>GAZ</oboInOwl:hasOBONamespace>
        <oboInOwl:id>GAZ:00046936</oboInOwl:id>
        <rdfs:label>Motuharakeke Island</rdfs:label>
    </owl:NamedIndividual>
    


    <!-- http://purl.obolibrary.org/obo/GAZ_00046937 -->

    <owl:NamedIndividual rdf:about="http://purl.obolibrary.org/obo/GAZ_00046937">
        <obo:RO_0001025 rdf:resource="http://purl.obolibrary.org/obo/GAZ_00046932"/>
        <obo:IAO_0000115>One of the Cavalli Islands.</obo:IAO_0000115>
        <oboInOwl:hasOBONamespace>GAZ</oboInOwl:hasOBONamespace>
        <oboInOwl:id>GAZ:00046937</oboInOwl:id>
        <rdfs:label>Panaki Island</rdfs:label>
    </owl:NamedIndividual>
    


    <!-- http://purl.obolibrary.org/obo/GAZ_00046938 -->

    <owl:NamedIndividual rdf:about="http://purl.obolibrary.org/obo/GAZ_00046938">
        <obo:RO_0001025 rdf:resource="http://purl.obolibrary.org/obo/GAZ_00046932"/>
        <obo:IAO_0000115>One of the Cavalli Islands.</obo:IAO_0000115>
        <oboInOwl:hasOBONamespace>GAZ</oboInOwl:hasOBONamespace>
        <oboInOwl:id>GAZ:00046938</oboInOwl:id>
        <rdfs:label>Nukutaunga Island</rdfs:label>
    </owl:NamedIndividual>
    


    <!-- http://purl.obolibrary.org/obo/GAZ_00046939 -->

    <owl:NamedIndividual rdf:about="http://purl.obolibrary.org/obo/GAZ_00046939">
        <obo:RO_0001025 rdf:resource="http://purl.obolibrary.org/obo/GAZ_00046932"/>
        <obo:IAO_0000115>One of the Cavalli Islands.</obo:IAO_0000115>
        <oboInOwl:hasOBONamespace>GAZ</oboInOwl:hasOBONamespace>
        <oboInOwl:id>GAZ:00046939</oboInOwl:id>
        <rdfs:label>Haraweka Island</rdfs:label>
    </owl:NamedIndividual>
    


    <!-- http://purl.obolibrary.org/obo/GAZ_00046940 -->

    <owl:NamedIndividual rdf:about="http://purl.obolibrary.org/obo/GAZ_00046940">
        <obo:RO_0001025 rdf:resource="http://purl.obolibrary.org/obo/GAZ_00008572"/>
        <obo:RO_0001025 rdf:resource="http://purl.obolibrary.org/obo/GAZ_00047047"/>
        <obo:IAO_0000115>A 514 ha island in the southwest of New Zealand, and is part of Fiordland National Park. It lies at the entrance to Chalky Inlet, at the southwestern tip of the South Island, ten km northwest of Puysegur Point, 15 km southeast of West Cape, and 140 km west of Invercargill.</obo:IAO_0000115>
        <oboInOwl:hasOBONamespace>GAZ</oboInOwl:hasOBONamespace>
        <oboInOwl:id>GAZ:00046940</oboInOwl:id>
        <rdfs:label>Chalky Island</rdfs:label>
    </owl:NamedIndividual>
    


    <!-- http://purl.obolibrary.org/obo/GAZ_00046943 -->

    <owl:NamedIndividual rdf:about="http://purl.obolibrary.org/obo/GAZ_00046943">
        <obo:RO_0001025 rdf:resource="http://purl.obolibrary.org/obo/GAZ_00046945"/>
        <obo:IAO_0000115>One of three channels connecting the Hauraki Gulf with the Pacific Ocean to the northeast of Auckland, New Zealand.</obo:IAO_0000115>
        <oboInOwl:hasOBONamespace>GAZ</oboInOwl:hasOBONamespace>
        <oboInOwl:id>GAZ:00046943</oboInOwl:id>
        <rdfs:label>Colville Channel</rdfs:label>
    </owl:NamedIndividual>
    


    <!-- http://purl.obolibrary.org/obo/GAZ_00046944 -->

    <owl:NamedIndividual rdf:about="http://purl.obolibrary.org/obo/GAZ_00046944">
        <obo:RO_0001025 rdf:resource="http://purl.obolibrary.org/obo/GAZ_00046943"/>
        <obo:IAO_0000115>A small island in the center of Colville Channel.</obo:IAO_0000115>
        <oboInOwl:hasOBONamespace>GAZ</oboInOwl:hasOBONamespace>
        <oboInOwl:id>GAZ:00046944</oboInOwl:id>
        <rdfs:label>Channel Island</rdfs:label>
    </owl:NamedIndividual>
    


    <!-- http://purl.obolibrary.org/obo/GAZ_00046945 -->

    <owl:NamedIndividual rdf:about="http://purl.obolibrary.org/obo/GAZ_00046945">
        <rdf:type rdf:resource="http://purl.obolibrary.org/obo/ENVO_00000032"/>
        <obo:RO_0001025 rdf:resource="http://purl.obolibrary.org/obo/GAZ_00004765"/>
        <obo:IAO_0000115>A gulf that lies between Auckland, the Coromandel Peninsula, and the Hauraki Plains.</obo:IAO_0000115>
        <oboInOwl:hasOBONamespace>GAZ</oboInOwl:hasOBONamespace>
        <oboInOwl:id>GAZ:00046945</oboInOwl:id>
        <rdfs:label>Hauraki Gulf</rdfs:label>
    </owl:NamedIndividual>
    


    <!-- http://purl.obolibrary.org/obo/GAZ_00046946 -->

    <owl:NamedIndividual rdf:about="http://purl.obolibrary.org/obo/GAZ_00046946">
        <rdf:type rdf:resource="http://purl.obolibrary.org/obo/ENVO_00000222"/>
        <obo:RO_0001025 rdf:resource="http://purl.obolibrary.org/obo/GAZ_00046945"/>
        <obo:IAO_0000115>A volcanic island in the Hauraki Gulf near Auckland, New Zealand. It is separated from the mainland of Auckland&apos;s North Shore by the Rangitoto Channel.</obo:IAO_0000115>
        <oboInOwl:hasOBONamespace>GAZ</oboInOwl:hasOBONamespace>
        <oboInOwl:id>GAZ:00046946</oboInOwl:id>
        <rdfs:label>Rangitoto Island</rdfs:label>
    </owl:NamedIndividual>
    


    <!-- http://purl.obolibrary.org/obo/GAZ_00046947 -->

    <owl:NamedIndividual rdf:about="http://purl.obolibrary.org/obo/GAZ_00046947">
        <obo:RO_0001025 rdf:resource="http://purl.obolibrary.org/obo/GAZ_00046945"/>
        <obo:IAO_0000115>An island in the Hauraki Gulf, an arm of the Pacific Ocean to the northeast of Auckland, New Zealand, north-east of Motutapu Island.</obo:IAO_0000115>
        <oboInOwl:hasOBONamespace>GAZ</oboInOwl:hasOBONamespace>
        <oboInOwl:id>GAZ:00046947</oboInOwl:id>
        <rdfs:label>Rakino Island</rdfs:label>
    </owl:NamedIndividual>
    


    <!-- http://purl.obolibrary.org/obo/GAZ_00046948 -->

    <owl:NamedIndividual rdf:about="http://purl.obolibrary.org/obo/GAZ_00046948">
        <obo:RO_0001025 rdf:resource="http://purl.obolibrary.org/obo/GAZ_00046945"/>
        <obo:IAO_0000115>An island that lies in the Hauraki Gulf of New Zealand, 4 km east of the Whangaparaoa Peninsula in the North Island and 30 km north east of Auckland.</obo:IAO_0000115>
        <oboInOwl:hasOBONamespace>GAZ</oboInOwl:hasOBONamespace>
        <oboInOwl:id>GAZ:00046948</oboInOwl:id>
        <rdfs:label>Tiritiri Matangi Island</rdfs:label>
    </owl:NamedIndividual>
    


    <!-- http://purl.obolibrary.org/obo/GAZ_00046949 -->

    <owl:NamedIndividual rdf:about="http://purl.obolibrary.org/obo/GAZ_00046949">
        <obo:RO_0001025 rdf:resource="http://purl.obolibrary.org/obo/GAZ_00046945"/>
        <obo:IAO_0000115>A small island SW of Ponui Island.</obo:IAO_0000115>
        <oboInOwl:hasOBONamespace>GAZ</oboInOwl:hasOBONamespace>
        <oboInOwl:id>GAZ:00046949</oboInOwl:id>
        <rdfs:label>Pakihi Island</rdfs:label>
    </owl:NamedIndividual>
    


    <!-- http://purl.obolibrary.org/obo/GAZ_00046950 -->

    <owl:NamedIndividual rdf:about="http://purl.obolibrary.org/obo/GAZ_00046950">
        <obo:RO_0001025 rdf:resource="http://purl.obolibrary.org/obo/GAZ_00046945"/>
        <obo:IAO_0000115>An island in the Hauraki Gulf of New Zealand.</obo:IAO_0000115>
        <oboInOwl:hasOBONamespace>GAZ</oboInOwl:hasOBONamespace>
        <oboInOwl:id>GAZ:00046950</oboInOwl:id>
        <rdfs:label>Pakatoa Island</rdfs:label>
    </owl:NamedIndividual>
    


    <!-- http://purl.obolibrary.org/obo/GAZ_00046951 -->

    <owl:NamedIndividual rdf:about="http://purl.obolibrary.org/obo/GAZ_00046951">
        <obo:RO_0001025 rdf:resource="http://purl.obolibrary.org/obo/GAZ_00046945"/>
        <obo:IAO_0000115>An island that lies east of Waiheke Island in the Hauraki Gulf of New Zealand.</obo:IAO_0000115>
        <oboInOwl:hasOBONamespace>GAZ</oboInOwl:hasOBONamespace>
        <oboInOwl:id>GAZ:00046951</oboInOwl:id>
        <rdfs:label>Rotoroa Island</rdfs:label>
    </owl:NamedIndividual>
    


    <!-- http://purl.obolibrary.org/obo/GAZ_00046953 -->

    <owl:NamedIndividual rdf:about="http://purl.obolibrary.org/obo/GAZ_00046953">
        <obo:RO_0001025 rdf:resource="http://purl.obolibrary.org/obo/GAZ_00046945"/>
        <obo:IAO_0000115>The northernmost of several small groups of islands that lie in the Hauraki Gulf off the west coast of the Coromandel Peninsula, New Zealand. They lie some five km to the southwest of Colville, and are uninhabited.</obo:IAO_0000115>
        <oboInOwl:hasOBONamespace>GAZ</oboInOwl:hasOBONamespace>
        <oboInOwl:id>GAZ:00046953</oboInOwl:id>
        <rdfs:label>Motukawao Islands</rdfs:label>
    </owl:NamedIndividual>
    


    <!-- http://purl.obolibrary.org/obo/GAZ_00046954 -->

    <owl:NamedIndividual rdf:about="http://purl.obolibrary.org/obo/GAZ_00046954">
        <obo:RO_0001025 rdf:resource="http://purl.obolibrary.org/obo/GAZ_00046945"/>
        <obo:IAO_0000115>A small Hauraki Gulf island north of Musick Point.</obo:IAO_0000115>
        <oboInOwl:hasOBONamespace>GAZ</oboInOwl:hasOBONamespace>
        <oboInOwl:id>GAZ:00046954</oboInOwl:id>
        <rdfs:label>Browns Island</rdfs:label>
    </owl:NamedIndividual>
    


    <!-- http://purl.obolibrary.org/obo/GAZ_00046955 -->

    <owl:NamedIndividual rdf:about="http://purl.obolibrary.org/obo/GAZ_00046955">
        <obo:RO_0001025 rdf:resource="http://purl.obolibrary.org/obo/GAZ_00046945"/>
        <obo:IAO_0000115>The largest of a small group of islands at the entrance to Coromandel harbour in the Hauraki Gulf, off the coast of New Zealand&apos;s North Island.</obo:IAO_0000115>
        <oboInOwl:hasOBONamespace>GAZ</oboInOwl:hasOBONamespace>
        <oboInOwl:id>GAZ:00046955</oboInOwl:id>
        <rdfs:label>Whanganui Island</rdfs:label>
    </owl:NamedIndividual>
    


    <!-- http://purl.obolibrary.org/obo/GAZ_00046959 -->

    <owl:NamedIndividual rdf:about="http://purl.obolibrary.org/obo/GAZ_00046959">
        <obo:RO_0001025 rdf:resource="http://purl.obolibrary.org/obo/GAZ_00046945"/>
        <obo:IAO_0000115>An island off the northeast coast of New Zealand&apos;s Great Barrier Island. It is located 95 km to the northeast of Auckland.</obo:IAO_0000115>
        <oboInOwl:hasOBONamespace>GAZ</oboInOwl:hasOBONamespace>
        <oboInOwl:id>GAZ:00046959</oboInOwl:id>
        <rdfs:label>Dragon Island</rdfs:label>
    </owl:NamedIndividual>
    


    <!-- http://purl.obolibrary.org/obo/GAZ_00046961 -->

    <owl:NamedIndividual rdf:about="http://purl.obolibrary.org/obo/GAZ_00046961">
        <obo:RO_0001025 rdf:resource="http://purl.obolibrary.org/obo/GAZ_00004760"/>
        <oboInOwl:hasOBONamespace>GAZ</oboInOwl:hasOBONamespace>
        <oboInOwl:id>GAZ:00046961</oboInOwl:id>
        <rdfs:label>Goat Island</rdfs:label>
    </owl:NamedIndividual>
    


    <!-- http://purl.obolibrary.org/obo/GAZ_00046962 -->

    <owl:NamedIndividual rdf:about="http://purl.obolibrary.org/obo/GAZ_00046962">
        <obo:RO_0001025 rdf:resource="http://purl.obolibrary.org/obo/GAZ_00047012"/>
        <obo:IAO_0000115>An island in Otago Harbour in Otago, in the southern South Island of New Zealand. It is located between Port Chalmers and Portobello, to the northeast of Dunedin&apos;s city centre.</obo:IAO_0000115>
        <oboInOwl:hasOBONamespace>GAZ</oboInOwl:hasOBONamespace>
        <oboInOwl:id>GAZ:00046962</oboInOwl:id>
        <rdfs:label>Goat Island</rdfs:label>
    </owl:NamedIndividual>
    


    <!-- http://purl.obolibrary.org/obo/GAZ_00046963 -->

    <owl:NamedIndividual rdf:about="http://purl.obolibrary.org/obo/GAZ_00046963">
        <obo:RO_0001025 rdf:resource="http://purl.obolibrary.org/obo/GAZ_00004768"/>
        <obo:IAO_0000115>A small uninhabited island located 13 km southwest of Dunedin, close to the mouth of the Kaikorai Lagoon.</obo:IAO_0000115>
        <oboInOwl:hasOBONamespace>GAZ</oboInOwl:hasOBONamespace>
        <oboInOwl:id>GAZ:00046963</oboInOwl:id>
        <rdfs:label>Green Island</rdfs:label>
    </owl:NamedIndividual>
    


    <!-- http://purl.obolibrary.org/obo/GAZ_00046973 -->

    <owl:NamedIndividual rdf:about="http://purl.obolibrary.org/obo/GAZ_00046973">
        <obo:RO_0001025 rdf:resource="http://purl.obolibrary.org/obo/GAZ_00046945"/>
        <obo:IAO_0000115>An island that lies off the northeastern coast of New Zealand&apos;s North Island. It is 80 km to the north of Auckland. The island is separated from the mainland to the west by Jellicoe Channel, and from the larger Great Barrier Island to the east by Cradock Channel. The island is an extinct andesitic volcanic cone.</obo:IAO_0000115>
        <oboInOwl:hasOBONamespace>GAZ</oboInOwl:hasOBONamespace>
        <oboInOwl:id>GAZ:00046973</oboInOwl:id>
        <rdfs:label>Little Barrier Island</rdfs:label>
    </owl:NamedIndividual>
    


    <!-- http://purl.obolibrary.org/obo/GAZ_00046974 -->

    <owl:NamedIndividual rdf:about="http://purl.obolibrary.org/obo/GAZ_00046974">
        <obo:RO_0001025 rdf:resource="http://purl.obolibrary.org/obo/GAZ_00029958"/>
        <obo:IAO_0000115>A small but conspicuous island about 8 km off the west coast of the lower North Island of New Zealand. The island is separated from the mainland by the Rauoterangi channel.</obo:IAO_0000115>
        <oboInOwl:hasOBONamespace>GAZ</oboInOwl:hasOBONamespace>
        <oboInOwl:id>GAZ:00046974</oboInOwl:id>
        <rdfs:label>Kapiti Island</rdfs:label>
    </owl:NamedIndividual>
    


    <!-- http://purl.obolibrary.org/obo/GAZ_00046975 -->

    <owl:NamedIndividual rdf:about="http://purl.obolibrary.org/obo/GAZ_00046975">
        <obo:RO_0001025 rdf:resource="http://purl.obolibrary.org/obo/GAZ_00046945"/>
        <obo:IAO_0000115>An island in the Hauraki Gulf, close to the north-eastern coast of the North Island of New Zealand. It lies 2 km off the coast of the North Auckland Peninsula, just south of Tawharanui Peninsula, and shelters Kawau Bay to the north-east of Warkworth. It is 50 km north of Auckland.</obo:IAO_0000115>
        <oboInOwl:hasOBONamespace>GAZ</oboInOwl:hasOBONamespace>
        <oboInOwl:id>GAZ:00046975</oboInOwl:id>
        <rdfs:label>Kawau Island</rdfs:label>
    </owl:NamedIndividual>
    


    <!-- http://purl.obolibrary.org/obo/GAZ_00046976 -->

    <owl:NamedIndividual rdf:about="http://purl.obolibrary.org/obo/GAZ_00046976">
        <obo:RO_0001025 rdf:resource="http://purl.obolibrary.org/obo/GAZ_00009760"/>
        <obo:RO_0001025 rdf:resource="http://purl.obolibrary.org/obo/GAZ_00046929"/>
        <obo:IAO_0000115>A large natural harbour on the southern tip of New Zealand&apos;s North Island. New Zealand&apos;s capital, Wellington, is located on the western side of Wellington Harbour. It is an arm of Cook Strait, with a two km wide entrance at its southern end between Pencarrow Head and the Miramar Peninsula.</obo:IAO_0000115>
        <oboInOwl:hasOBONamespace>GAZ</oboInOwl:hasOBONamespace>
        <oboInOwl:id>GAZ:00046976</oboInOwl:id>
        <rdfs:label>Wellington Harbor</rdfs:label>
    </owl:NamedIndividual>
    


    <!-- http://purl.obolibrary.org/obo/GAZ_00046977 -->

    <owl:NamedIndividual rdf:about="http://purl.obolibrary.org/obo/GAZ_00046977">
        <obo:RO_0001025 rdf:resource="http://purl.obolibrary.org/obo/GAZ_00046976"/>
        <oboInOwl:hasOBONamespace>GAZ</oboInOwl:hasOBONamespace>
        <oboInOwl:id>GAZ:00046977</oboInOwl:id>
        <rdfs:label>Makaro island</rdfs:label>
    </owl:NamedIndividual>
    


    <!-- http://purl.obolibrary.org/obo/GAZ_00046978 -->

    <owl:NamedIndividual rdf:about="http://purl.obolibrary.org/obo/GAZ_00046978">
        <obo:RO_0001025 rdf:resource="http://purl.obolibrary.org/obo/GAZ_00046976"/>
        <oboInOwl:hasOBONamespace>GAZ</oboInOwl:hasOBONamespace>
        <oboInOwl:id>GAZ:00046978</oboInOwl:id>
        <rdfs:label>Matiu Island</rdfs:label>
    </owl:NamedIndividual>
    


    <!-- http://purl.obolibrary.org/obo/GAZ_00046979 -->

    <owl:NamedIndividual rdf:about="http://purl.obolibrary.org/obo/GAZ_00046979">
        <obo:RO_0001025 rdf:resource="http://purl.obolibrary.org/obo/GAZ_00008565"/>
        <obo:IAO_0000115>The smaller of two islands that lie off the southwest coast of the North Island of New Zealand (the larger is Kapiti Island).</obo:IAO_0000115>
        <oboInOwl:hasOBONamespace>GAZ</oboInOwl:hasOBONamespace>
        <oboInOwl:id>GAZ:00046979</oboInOwl:id>
        <rdfs:label>Mana Island</rdfs:label>
    </owl:NamedIndividual>
    


    <!-- http://purl.obolibrary.org/obo/GAZ_00046980 -->

    <owl:NamedIndividual rdf:about="http://purl.obolibrary.org/obo/GAZ_00046980">
        <obo:RO_0001025 rdf:resource="http://purl.obolibrary.org/obo/GAZ_00030230"/>
        <obo:IAO_0000115>An island located in the western Bay of Plenty in New Zealand&apos;s North Island. A long, flat island, it is 20 km in length but rarely more than three km wide.</obo:IAO_0000115>
        <oboInOwl:hasOBONamespace>GAZ</oboInOwl:hasOBONamespace>
        <oboInOwl:id>GAZ:00046980</oboInOwl:id>
        <rdfs:label>Matakana Island</rdfs:label>
    </owl:NamedIndividual>
    


    <!-- http://purl.obolibrary.org/obo/GAZ_00046981 -->

    <owl:NamedIndividual rdf:about="http://purl.obolibrary.org/obo/GAZ_00046981">
        <obo:RO_0001025 rdf:resource="http://purl.obolibrary.org/obo/GAZ_00046925"/>
        <oboInOwl:hasOBONamespace>GAZ</oboInOwl:hasOBONamespace>
        <oboInOwl:id>GAZ:00046981</oboInOwl:id>
        <rdfs:label>Maud Island</rdfs:label>
    </owl:NamedIndividual>
    


    <!-- http://purl.obolibrary.org/obo/GAZ_00046983 -->

    <owl:NamedIndividual rdf:about="http://purl.obolibrary.org/obo/GAZ_00046983">
        <obo:RO_0001025 rdf:resource="http://purl.obolibrary.org/obo/GAZ_00046953"/>
        <obo:IAO_0000115>One of the Motukawao Islands.</obo:IAO_0000115>
        <oboInOwl:hasOBONamespace>GAZ</oboInOwl:hasOBONamespace>
        <oboInOwl:id>GAZ:00046983</oboInOwl:id>
        <rdfs:label>Motuwi Island</rdfs:label>
    </owl:NamedIndividual>
    


    <!-- http://purl.obolibrary.org/obo/GAZ_00046984 -->

    <owl:NamedIndividual rdf:about="http://purl.obolibrary.org/obo/GAZ_00046984">
        <obo:RO_0001025 rdf:resource="http://purl.obolibrary.org/obo/GAZ_00046953"/>
        <obo:IAO_0000115>One of the Motukawao Islands.</obo:IAO_0000115>
        <oboInOwl:hasOBONamespace>GAZ</oboInOwl:hasOBONamespace>
        <oboInOwl:id>GAZ:00046984</oboInOwl:id>
        <rdfs:label>Ngamotukaraka Island</rdfs:label>
    </owl:NamedIndividual>
    


    <!-- http://purl.obolibrary.org/obo/GAZ_00046985 -->

    <owl:NamedIndividual rdf:about="http://purl.obolibrary.org/obo/GAZ_00046985">
        <obo:RO_0001025 rdf:resource="http://purl.obolibrary.org/obo/GAZ_00046953"/>
        <obo:IAO_0000115>One of the Motukawao Islands.</obo:IAO_0000115>
        <oboInOwl:hasOBONamespace>GAZ</oboInOwl:hasOBONamespace>
        <oboInOwl:id>GAZ:00046985</oboInOwl:id>
        <rdfs:label>Moturua Island</rdfs:label>
    </owl:NamedIndividual>
    


    <!-- http://purl.obolibrary.org/obo/GAZ_00046986 -->

    <owl:NamedIndividual rdf:about="http://purl.obolibrary.org/obo/GAZ_00046986">
        <obo:RO_0001025 rdf:resource="http://purl.obolibrary.org/obo/GAZ_00046953"/>
        <obo:IAO_0000115>One of the Motukawao Islands.</obo:IAO_0000115>
        <oboInOwl:hasOBONamespace>GAZ</oboInOwl:hasOBONamespace>
        <oboInOwl:id>GAZ:00046986</oboInOwl:id>
        <rdfs:label>Motukaramarama Island</rdfs:label>
    </owl:NamedIndividual>
    


    <!-- http://purl.obolibrary.org/obo/GAZ_00046987 -->

    <owl:NamedIndividual rdf:about="http://purl.obolibrary.org/obo/GAZ_00046987">
        <obo:RO_0001025 rdf:resource="http://purl.obolibrary.org/obo/GAZ_00008562"/>
        <obo:IAO_0000115>A small off shore island in North Canterbury.</obo:IAO_0000115>
        <oboInOwl:hasOBONamespace>GAZ</oboInOwl:hasOBONamespace>
        <oboInOwl:id>GAZ:00046987</oboInOwl:id>
        <rdfs:label>Motunau Island</rdfs:label>
    </owl:NamedIndividual>
    


    <!-- http://purl.obolibrary.org/obo/GAZ_00046988 -->

    <owl:NamedIndividual rdf:about="http://purl.obolibrary.org/obo/GAZ_00046988">
        <obo:RO_0001025 rdf:resource="http://purl.obolibrary.org/obo/GAZ_00004767"/>
        <oboInOwl:hasOBONamespace>GAZ</oboInOwl:hasOBONamespace>
        <oboInOwl:id>GAZ:00046988</oboInOwl:id>
        <rdfs:label>Taieri Island</rdfs:label>
    </owl:NamedIndividual>
    


    <!-- http://purl.obolibrary.org/obo/GAZ_00046989 -->

    <owl:NamedIndividual rdf:about="http://purl.obolibrary.org/obo/GAZ_00046989">
        <obo:RO_0001025 rdf:resource="http://purl.obolibrary.org/obo/GAZ_00046945"/>
        <obo:IAO_0000115>An island located in the Hauraki Gulf to the northeast of the city of Auckland, New Zealand.</obo:IAO_0000115>
        <oboInOwl:hasOBONamespace>GAZ</oboInOwl:hasOBONamespace>
        <oboInOwl:id>GAZ:00046989</oboInOwl:id>
        <rdfs:label>Motutapu Island</rdfs:label>
    </owl:NamedIndividual>
    


    <!-- http://purl.obolibrary.org/obo/GAZ_00046994 -->

    <owl:NamedIndividual rdf:about="http://purl.obolibrary.org/obo/GAZ_00046994">
        <obo:RO_0001025 rdf:resource="http://purl.obolibrary.org/obo/GAZ_00046945"/>
        <obo:IAO_0000115>An island located in the Hauraki Gulf, to the east of the city of Auckland, New Zealand. It is located to the southeast of Waiheke Island, at the eastern end of the Tamaki Strait, which separates the island from the Hunua Ranges on the mainland to the south.</obo:IAO_0000115>
        <oboInOwl:hasOBONamespace>GAZ</oboInOwl:hasOBONamespace>
        <oboInOwl:id>GAZ:00046994</oboInOwl:id>
        <rdfs:label>Ponui Island</rdfs:label>
    </owl:NamedIndividual>
    


    <!-- http://purl.obolibrary.org/obo/GAZ_00046995 -->

    <owl:NamedIndividual rdf:about="http://purl.obolibrary.org/obo/GAZ_00046995">
        <obo:RO_0001025 rdf:resource="http://purl.obolibrary.org/obo/GAZ_00004765"/>
        <obo:IAO_0000115>A small island off the southern tip of the Mahia Peninsula on the North Island of New Zealand.</obo:IAO_0000115>
        <oboInOwl:hasOBONamespace>GAZ</oboInOwl:hasOBONamespace>
        <oboInOwl:id>GAZ:00046995</oboInOwl:id>
        <rdfs:label>Portland Island</rdfs:label>
    </owl:NamedIndividual>
    


    <!-- http://purl.obolibrary.org/obo/GAZ_00046996 -->

    <owl:NamedIndividual rdf:about="http://purl.obolibrary.org/obo/GAZ_00046996">
        <obo:RO_0001025 rdf:resource="http://purl.obolibrary.org/obo/GAZ_00004765"/>
        <obo:IAO_0000115>A bay on the East Coast of New Zealand&apos;s North Island.</obo:IAO_0000115>
        <oboInOwl:hasOBONamespace>GAZ</oboInOwl:hasOBONamespace>
        <oboInOwl:id>GAZ:00046996</oboInOwl:id>
        <rdfs:label>Tolaga Bay</rdfs:label>
    </owl:NamedIndividual>
    


    <!-- http://purl.obolibrary.org/obo/GAZ_00046997 -->

    <owl:NamedIndividual rdf:about="http://purl.obolibrary.org/obo/GAZ_00046997">
        <obo:RO_0001025 rdf:resource="http://purl.obolibrary.org/obo/GAZ_00046996"/>
        <obo:IAO_0000115>An island that lies in Tolaga Bay, just offshore from Cook&apos;s Cove in New Zealand.</obo:IAO_0000115>
        <oboInOwl:hasOBONamespace>GAZ</oboInOwl:hasOBONamespace>
        <oboInOwl:id>GAZ:00046997</oboInOwl:id>
        <rdfs:label>Pourewa Island</rdfs:label>
    </owl:NamedIndividual>
    


    <!-- http://purl.obolibrary.org/obo/GAZ_00046998 -->

    <owl:NamedIndividual rdf:about="http://purl.obolibrary.org/obo/GAZ_00046998">
        <obo:RO_0001025 rdf:resource="http://purl.obolibrary.org/obo/GAZ_00029963"/>
        <obo:IAO_0000115>An inlet S of Christchurch and being the N border of the Banks Peninsula. It extends from the S end of Pegasus Bay.</obo:IAO_0000115>
        <oboInOwl:hasOBONamespace>GAZ</oboInOwl:hasOBONamespace>
        <oboInOwl:id>GAZ:00046998</oboInOwl:id>
        <rdfs:label>Lyttelton Harbour</rdfs:label>
    </owl:NamedIndividual>
    


    <!-- http://purl.obolibrary.org/obo/GAZ_00046999 -->

    <owl:NamedIndividual rdf:about="http://purl.obolibrary.org/obo/GAZ_00046999">
        <obo:RO_0001025 rdf:resource="http://purl.obolibrary.org/obo/GAZ_00046998"/>
        <obo:IAO_0000115>A small uninhabited island within Lyttelton Harbour in the South Island of New Zealand, close to Christchurch.</obo:IAO_0000115>
        <oboInOwl:hasOBONamespace>GAZ</oboInOwl:hasOBONamespace>
        <oboInOwl:id>GAZ:00046999</oboInOwl:id>
        <rdfs:label>Quail Island</rdfs:label>
    </owl:NamedIndividual>
    


    <!-- http://purl.obolibrary.org/obo/GAZ_00047000 -->

    <owl:NamedIndividual rdf:about="http://purl.obolibrary.org/obo/GAZ_00047000">
        <obo:RO_0001025 rdf:resource="http://purl.obolibrary.org/obo/GAZ_00008563"/>
        <obo:IAO_0000115>A large V-shaped bay at the north end of New Zealand&apos;s South Island. Located in the centre of the island&apos;s northern coast, it stretches along 120 km of coastline and is 70 km across at its widest point. It is an arm of the Tasman Sea, lying on the western approach to Cook Strait.</obo:IAO_0000115>
        <oboInOwl:hasOBONamespace>GAZ</oboInOwl:hasOBONamespace>
        <oboInOwl:id>GAZ:00047000</oboInOwl:id>
        <rdfs:label>Tasman Bay</rdfs:label>
    </owl:NamedIndividual>
    


    <!-- http://purl.obolibrary.org/obo/GAZ_00047001 -->

    <owl:NamedIndividual rdf:about="http://purl.obolibrary.org/obo/GAZ_00047001">
        <obo:RO_0001025 rdf:resource="http://purl.obolibrary.org/obo/GAZ_00047000"/>
        <obo:IAO_0000115>An island which lies across the southernmost part of Tasman Bay, at the top of New Zealand&apos;s South Island. The long narrow island runs east-west for eight km, and covers 15 km2.</obo:IAO_0000115>
        <oboInOwl:hasOBONamespace>GAZ</oboInOwl:hasOBONamespace>
        <oboInOwl:id>GAZ:00047001</oboInOwl:id>
        <rdfs:label>Rabbit Island</rdfs:label>
    </owl:NamedIndividual>
    


    <!-- http://purl.obolibrary.org/obo/GAZ_00047002 -->

    <owl:NamedIndividual rdf:about="http://purl.obolibrary.org/obo/GAZ_00047002">
        <obo:RO_0001025 rdf:resource="http://purl.obolibrary.org/obo/GAZ_00046945"/>
        <oboInOwl:hasOBONamespace>GAZ</oboInOwl:hasOBONamespace>
        <oboInOwl:id>GAZ:00047002</oboInOwl:id>
        <rdfs:label>Rabbit Island</rdfs:label>
    </owl:NamedIndividual>
    


    <!-- http://purl.obolibrary.org/obo/GAZ_00047003 -->

    <owl:NamedIndividual rdf:about="http://purl.obolibrary.org/obo/GAZ_00047003">
        <obo:RO_0001025 rdf:resource="http://purl.obolibrary.org/obo/GAZ_00004781"/>
        <oboInOwl:hasOBONamespace>GAZ</oboInOwl:hasOBONamespace>
        <oboInOwl:id>GAZ:00047003</oboInOwl:id>
        <rdfs:label>Rabbit Island</rdfs:label>
    </owl:NamedIndividual>
    


    <!-- http://purl.obolibrary.org/obo/GAZ_00047004 -->

    <owl:NamedIndividual rdf:about="http://purl.obolibrary.org/obo/GAZ_00047004">
        <obo:RO_0001025 rdf:resource="http://purl.obolibrary.org/obo/GAZ_00030230"/>
        <oboInOwl:hasOBONamespace>GAZ</oboInOwl:hasOBONamespace>
        <oboInOwl:id>GAZ:00047004</oboInOwl:id>
        <rdfs:label>Rabbit Island</rdfs:label>
    </owl:NamedIndividual>
    


    <!-- http://purl.obolibrary.org/obo/GAZ_00047005 -->

    <owl:NamedIndividual rdf:about="http://purl.obolibrary.org/obo/GAZ_00047005">
        <obo:RO_0001025 rdf:resource="http://purl.obolibrary.org/obo/GAZ_00000469"/>
        <obo:IAO_0000115>A strait between the South Island, New Zealand on the north side, with the three large bays Te Waewae Bay, Oreti Beach and Toetoes Bay, and the Solander Islands, Stewart Island/Rakiura and Ruapuke Island on the south.</obo:IAO_0000115>
        <oboInOwl:hasOBONamespace>GAZ</oboInOwl:hasOBONamespace>
        <oboInOwl:id>GAZ:00047005</oboInOwl:id>
        <rdfs:label>Foveaux Strait</rdfs:label>
    </owl:NamedIndividual>
    


    <!-- http://purl.obolibrary.org/obo/GAZ_00047006 -->

    <owl:NamedIndividual rdf:about="http://purl.obolibrary.org/obo/GAZ_00047006">
        <obo:RO_0001025 rdf:resource="http://purl.obolibrary.org/obo/GAZ_00047005"/>
        <oboInOwl:hasOBONamespace>GAZ</oboInOwl:hasOBONamespace>
        <oboInOwl:id>GAZ:00047006</oboInOwl:id>
        <rdfs:label>Rabbit Island</rdfs:label>
    </owl:NamedIndividual>
    


    <!-- http://purl.obolibrary.org/obo/GAZ_00047007 -->

    <owl:NamedIndividual rdf:about="http://purl.obolibrary.org/obo/GAZ_00047007">
        <obo:RO_0001025 rdf:resource="http://purl.obolibrary.org/obo/GAZ_00007177"/>
        <oboInOwl:hasOBONamespace>GAZ</oboInOwl:hasOBONamespace>
        <oboInOwl:id>GAZ:00047007</oboInOwl:id>
        <rdfs:label>Solander Island</rdfs:label>
    </owl:NamedIndividual>
    


    <!-- http://purl.obolibrary.org/obo/GAZ_00047008 -->

    <owl:NamedIndividual rdf:about="http://purl.obolibrary.org/obo/GAZ_00047008">
        <obo:RO_0001025 rdf:resource="http://purl.obolibrary.org/obo/GAZ_00007177"/>
        <oboInOwl:hasOBONamespace>GAZ</oboInOwl:hasOBONamespace>
        <oboInOwl:id>GAZ:00047008</oboInOwl:id>
        <rdfs:label>Little Solander Island</rdfs:label>
    </owl:NamedIndividual>
    


    <!-- http://purl.obolibrary.org/obo/GAZ_00047009 -->

    <owl:NamedIndividual rdf:about="http://purl.obolibrary.org/obo/GAZ_00047009">
        <obo:RO_0001025 rdf:resource="http://purl.obolibrary.org/obo/GAZ_00007177"/>
        <oboInOwl:hasOBONamespace>GAZ</oboInOwl:hasOBONamespace>
        <oboInOwl:id>GAZ:00047009</oboInOwl:id>
        <rdfs:label>Pierced Rock</rdfs:label>
    </owl:NamedIndividual>
    


    <!-- http://purl.obolibrary.org/obo/GAZ_00047010 -->

    <owl:NamedIndividual rdf:about="http://purl.obolibrary.org/obo/GAZ_00047010">
        <obo:RO_0001025 rdf:resource="http://purl.obolibrary.org/obo/GAZ_00047005"/>
        <obo:IAO_0000115>One of the southernmost islands in New Zealand&apos;s main chain of islands. It lies 15 km to the southeast of Bluff and 32 km northeast of Oban on Stewart Island/Rakiura.</obo:IAO_0000115>
        <oboInOwl:hasOBONamespace>GAZ</oboInOwl:hasOBONamespace>
        <oboInOwl:id>GAZ:00047010</oboInOwl:id>
        <rdfs:label>Ruapuke Island</rdfs:label>
    </owl:NamedIndividual>
    


    <!-- http://purl.obolibrary.org/obo/GAZ_00047012 -->

    <owl:NamedIndividual rdf:about="http://purl.obolibrary.org/obo/GAZ_00047012">
        <obo:RO_0001025 rdf:resource="http://purl.obolibrary.org/obo/GAZ_00004767"/>
        <obo:IAO_0000115>A long, much-indented stretch of generally navigable water separating Otago Peninsula from the main urban areas of Dunedin, New Zealand.</obo:IAO_0000115>
        <oboInOwl:hasOBONamespace>GAZ</oboInOwl:hasOBONamespace>
        <oboInOwl:id>GAZ:00047012</oboInOwl:id>
        <rdfs:label>Otago Harbour</rdfs:label>
    </owl:NamedIndividual>
    


    <!-- http://purl.obolibrary.org/obo/GAZ_00047013 -->

    <owl:NamedIndividual rdf:about="http://purl.obolibrary.org/obo/GAZ_00047013">
        <obo:RO_0001025 rdf:resource="http://purl.obolibrary.org/obo/GAZ_00047012"/>
        <obo:IAO_0000115>The largest island in Otago Harbour, close to the city of Dunedin, New Zealand.</obo:IAO_0000115>
        <oboInOwl:hasOBONamespace>GAZ</oboInOwl:hasOBONamespace>
        <oboInOwl:id>GAZ:00047013</oboInOwl:id>
        <rdfs:label>Quarantine Island</rdfs:label>
    </owl:NamedIndividual>
    


    <!-- http://purl.obolibrary.org/obo/GAZ_00047014 -->

    <owl:NamedIndividual rdf:about="http://purl.obolibrary.org/obo/GAZ_00047014">
        <obo:RO_0001025 rdf:resource="http://purl.obolibrary.org/obo/GAZ_00047012"/>
        <obo:IAO_0000115>A small island in Otago Harbour.</obo:IAO_0000115>
        <oboInOwl:hasOBONamespace>GAZ</oboInOwl:hasOBONamespace>
        <oboInOwl:id>GAZ:00047014</oboInOwl:id>
        <rdfs:label>Pudding Island</rdfs:label>
    </owl:NamedIndividual>
    


    <!-- http://purl.obolibrary.org/obo/GAZ_00047015 -->

    <owl:NamedIndividual rdf:about="http://purl.obolibrary.org/obo/GAZ_00047015">
        <obo:RO_0001025 rdf:resource="http://purl.obolibrary.org/obo/GAZ_00047047"/>
        <obo:IAO_0000115>An island in southwestern New Zealand. It lies entirely within Fiordland National Park. Roughly triangular in shape, it lies between Doubtful Sound in the south and Thompson Sound in the north, with its west coast facing the Tasman Sea.</obo:IAO_0000115>
        <oboInOwl:hasOBONamespace>GAZ</oboInOwl:hasOBONamespace>
        <oboInOwl:id>GAZ:00047015</oboInOwl:id>
        <rdfs:label>Secretary Island</rdfs:label>
    </owl:NamedIndividual>
    


    <!-- http://purl.obolibrary.org/obo/GAZ_00047017 -->

    <owl:NamedIndividual rdf:about="http://purl.obolibrary.org/obo/GAZ_00047017">
        <obo:RO_0001025 rdf:resource="http://purl.obolibrary.org/obo/GAZ_00046925"/>
        <obo:IAO_0000115>An island at the northern most tip of the Marlborough Sounds in the South Island of New Zealand.</obo:IAO_0000115>
        <oboInOwl:hasOBONamespace>GAZ</oboInOwl:hasOBONamespace>
        <oboInOwl:id>GAZ:00047017</oboInOwl:id>
        <rdfs:label>Stephens Island</rdfs:label>
    </owl:NamedIndividual>
    


    <!-- http://purl.obolibrary.org/obo/GAZ_00047018 -->

    <owl:NamedIndividual rdf:about="http://purl.obolibrary.org/obo/GAZ_00047018">
        <obo:RO_0001025 rdf:resource="http://purl.obolibrary.org/obo/GAZ_00142739"/>
        <obo:IAO_0000115>A bay on the Cook Strait.</obo:IAO_0000115>
        <oboInOwl:hasOBONamespace>GAZ</oboInOwl:hasOBONamespace>
        <oboInOwl:id>GAZ:00047018</oboInOwl:id>
        <rdfs:label>Island Bay</rdfs:label>
    </owl:NamedIndividual>
    


    <!-- http://purl.obolibrary.org/obo/GAZ_00047019 -->

    <owl:NamedIndividual rdf:about="http://purl.obolibrary.org/obo/GAZ_00047019">
        <obo:RO_0001025 rdf:resource="http://purl.obolibrary.org/obo/GAZ_00047018"/>
        <obo:IAO_0000115>An island.</obo:IAO_0000115>
        <oboInOwl:hasOBONamespace>GAZ</oboInOwl:hasOBONamespace>
        <oboInOwl:id>GAZ:00047019</oboInOwl:id>
        <rdfs:label>Tapu Te Ranga Motu</rdfs:label>
    </owl:NamedIndividual>
    


    <!-- http://purl.obolibrary.org/obo/GAZ_00047020 -->

    <owl:NamedIndividual rdf:about="http://purl.obolibrary.org/obo/GAZ_00047020">
        <obo:RO_0001025 rdf:resource="http://purl.obolibrary.org/obo/GAZ_00008572"/>
        <obo:IAO_0000115>An island chain located to the southwest of Stewart Island.</obo:IAO_0000115>
        <oboInOwl:hasOBONamespace>GAZ</oboInOwl:hasOBONamespace>
        <oboInOwl:id>GAZ:00047020</oboInOwl:id>
        <rdfs:label>Southwestern Muttonbird Islands</rdfs:label>
    </owl:NamedIndividual>
    


    <!-- http://purl.obolibrary.org/obo/GAZ_00047021 -->

    <owl:NamedIndividual rdf:about="http://purl.obolibrary.org/obo/GAZ_00047021">
        <obo:RO_0001025 rdf:resource="http://purl.obolibrary.org/obo/GAZ_00008572"/>
        <obo:RO_0001025 rdf:resource="http://purl.obolibrary.org/obo/GAZ_00047005"/>
        <obo:IAO_0000115>An island chain located in Foveaux Strait, to the northeast of Stewart Island, between it and Ruapuke Island.</obo:IAO_0000115>
        <oboInOwl:hasOBONamespace>GAZ</oboInOwl:hasOBONamespace>
        <oboInOwl:id>GAZ:00047021</oboInOwl:id>
        <rdfs:label>Northeastern Mutton Bird Islands</rdfs:label>
    </owl:NamedIndividual>
    


    <!-- http://purl.obolibrary.org/obo/GAZ_00047022 -->

    <owl:NamedIndividual rdf:about="http://purl.obolibrary.org/obo/GAZ_00047022">
        <obo:RO_0001025 rdf:resource="http://purl.obolibrary.org/obo/GAZ_00047021"/>
        <oboInOwl:hasOBONamespace>GAZ</oboInOwl:hasOBONamespace>
        <oboInOwl:id>GAZ:00047022</oboInOwl:id>
        <rdfs:label>Fish Rock</rdfs:label>
    </owl:NamedIndividual>
    


    <!-- http://purl.obolibrary.org/obo/GAZ_00047023 -->

    <owl:NamedIndividual rdf:about="http://purl.obolibrary.org/obo/GAZ_00047023">
        <obo:RO_0001025 rdf:resource="http://purl.obolibrary.org/obo/GAZ_00047020"/>
        <oboInOwl:hasOBONamespace>GAZ</oboInOwl:hasOBONamespace>
        <oboInOwl:id>GAZ:00047023</oboInOwl:id>
        <rdfs:label>The Putauhina Nuggets</rdfs:label>
    </owl:NamedIndividual>
    


    <!-- http://purl.obolibrary.org/obo/GAZ_00047024 -->

    <owl:NamedIndividual rdf:about="http://purl.obolibrary.org/obo/GAZ_00047024">
        <obo:RO_0001025 rdf:resource="http://purl.obolibrary.org/obo/GAZ_00047021"/>
        <oboInOwl:hasOBONamespace>GAZ</oboInOwl:hasOBONamespace>
        <oboInOwl:id>GAZ:00047024</oboInOwl:id>
        <rdfs:label>The Bunker Islets</rdfs:label>
    </owl:NamedIndividual>
    


    <!-- http://purl.obolibrary.org/obo/GAZ_00047025 -->

    <owl:NamedIndividual rdf:about="http://purl.obolibrary.org/obo/GAZ_00047025">
        <obo:RO_0001025 rdf:resource="http://purl.obolibrary.org/obo/GAZ_00047021"/>
        <oboInOwl:hasOBONamespace>GAZ</oboInOwl:hasOBONamespace>
        <oboInOwl:id>GAZ:00047025</oboInOwl:id>
        <rdfs:label>Herekopare Island</rdfs:label>
    </owl:NamedIndividual>
    


    <!-- http://purl.obolibrary.org/obo/GAZ_00047026 -->

    <owl:NamedIndividual rdf:about="http://purl.obolibrary.org/obo/GAZ_00047026">
        <obo:RO_0001025 rdf:resource="http://purl.obolibrary.org/obo/GAZ_00047021"/>
        <oboInOwl:hasOBONamespace>GAZ</oboInOwl:hasOBONamespace>
        <oboInOwl:id>GAZ:00047026</oboInOwl:id>
        <rdfs:label>Edwards Island</rdfs:label>
    </owl:NamedIndividual>
    


    <!-- http://purl.obolibrary.org/obo/GAZ_00047027 -->

    <owl:NamedIndividual rdf:about="http://purl.obolibrary.org/obo/GAZ_00047027">
        <obo:RO_0001025 rdf:resource="http://purl.obolibrary.org/obo/GAZ_00047021"/>
        <oboInOwl:hasOBONamespace>GAZ</oboInOwl:hasOBONamespace>
        <oboInOwl:id>GAZ:00047027</oboInOwl:id>
        <rdfs:label>Jacky Lee Island</rdfs:label>
    </owl:NamedIndividual>
    


    <!-- http://purl.obolibrary.org/obo/GAZ_00047028 -->

    <owl:NamedIndividual rdf:about="http://purl.obolibrary.org/obo/GAZ_00047028">
        <obo:RO_0001025 rdf:resource="http://purl.obolibrary.org/obo/GAZ_00047021"/>
        <oboInOwl:hasOBONamespace>GAZ</oboInOwl:hasOBONamespace>
        <oboInOwl:id>GAZ:00047028</oboInOwl:id>
        <rdfs:label>Womens Island</rdfs:label>
    </owl:NamedIndividual>
    


    <!-- http://purl.obolibrary.org/obo/GAZ_00047029 -->

    <owl:NamedIndividual rdf:about="http://purl.obolibrary.org/obo/GAZ_00047029">
        <obo:RO_0001025 rdf:resource="http://purl.obolibrary.org/obo/GAZ_00047021"/>
        <oboInOwl:hasOBONamespace>GAZ</oboInOwl:hasOBONamespace>
        <oboInOwl:id>GAZ:00047029</oboInOwl:id>
        <rdfs:label>Kanetetoe Island</rdfs:label>
    </owl:NamedIndividual>
    


    <!-- http://purl.obolibrary.org/obo/GAZ_00047030 -->

    <owl:NamedIndividual rdf:about="http://purl.obolibrary.org/obo/GAZ_00047030">
        <obo:RO_0001025 rdf:resource="http://purl.obolibrary.org/obo/GAZ_00047021"/>
        <oboInOwl:hasOBONamespace>GAZ</oboInOwl:hasOBONamespace>
        <oboInOwl:id>GAZ:00047030</oboInOwl:id>
        <rdfs:label>North Island</rdfs:label>
    </owl:NamedIndividual>
    


    <!-- http://purl.obolibrary.org/obo/GAZ_00047031 -->

    <owl:NamedIndividual rdf:about="http://purl.obolibrary.org/obo/GAZ_00047031">
        <obo:RO_0001025 rdf:resource="http://purl.obolibrary.org/obo/GAZ_00047020"/>
        <oboInOwl:hasOBONamespace>GAZ</oboInOwl:hasOBONamespace>
        <oboInOwl:id>GAZ:00047031</oboInOwl:id>
        <rdfs:label>Tamaitemioka Island</rdfs:label>
    </owl:NamedIndividual>
    


    <!-- http://purl.obolibrary.org/obo/GAZ_00047032 -->

    <owl:NamedIndividual rdf:about="http://purl.obolibrary.org/obo/GAZ_00047032">
        <obo:RO_0001025 rdf:resource="http://purl.obolibrary.org/obo/GAZ_00047020"/>
        <oboInOwl:hasOBONamespace>GAZ</oboInOwl:hasOBONamespace>
        <oboInOwl:id>GAZ:00047032</oboInOwl:id>
        <rdfs:label>Pukaparara Island</rdfs:label>
    </owl:NamedIndividual>
    


    <!-- http://purl.obolibrary.org/obo/GAZ_00047033 -->

    <owl:NamedIndividual rdf:about="http://purl.obolibrary.org/obo/GAZ_00047033">
        <obo:RO_0001025 rdf:resource="http://purl.obolibrary.org/obo/GAZ_00047020"/>
        <oboInOwl:hasOBONamespace>GAZ</oboInOwl:hasOBONamespace>
        <oboInOwl:id>GAZ:00047033</oboInOwl:id>
        <rdfs:label>Little Moggy Island</rdfs:label>
    </owl:NamedIndividual>
    


    <!-- http://purl.obolibrary.org/obo/GAZ_00047034 -->

    <owl:NamedIndividual rdf:about="http://purl.obolibrary.org/obo/GAZ_00047034">
        <obo:RO_0001025 rdf:resource="http://purl.obolibrary.org/obo/GAZ_00047020"/>
        <oboInOwl:hasOBONamespace>GAZ</oboInOwl:hasOBONamespace>
        <oboInOwl:id>GAZ:00047034</oboInOwl:id>
        <rdfs:label>Kaimohu Island</rdfs:label>
    </owl:NamedIndividual>
    


    <!-- http://purl.obolibrary.org/obo/GAZ_00047035 -->

    <owl:NamedIndividual rdf:about="http://purl.obolibrary.org/obo/GAZ_00047035">
        <obo:RO_0001025 rdf:resource="http://purl.obolibrary.org/obo/GAZ_00047020"/>
        <oboInOwl:hasOBONamespace>GAZ</oboInOwl:hasOBONamespace>
        <oboInOwl:id>GAZ:00047035</oboInOwl:id>
        <rdfs:label>Pohowaitai Island</rdfs:label>
    </owl:NamedIndividual>
    


    <!-- http://purl.obolibrary.org/obo/GAZ_00047036 -->

    <owl:NamedIndividual rdf:about="http://purl.obolibrary.org/obo/GAZ_00047036">
        <obo:RO_0001025 rdf:resource="http://purl.obolibrary.org/obo/GAZ_00047020"/>
        <oboInOwl:hasOBONamespace>GAZ</oboInOwl:hasOBONamespace>
        <oboInOwl:id>GAZ:00047036</oboInOwl:id>
        <rdfs:label>Putauhina Island</rdfs:label>
    </owl:NamedIndividual>
    


    <!-- http://purl.obolibrary.org/obo/GAZ_00047037 -->

    <owl:NamedIndividual rdf:about="http://purl.obolibrary.org/obo/GAZ_00047037">
        <obo:RO_0001025 rdf:resource="http://purl.obolibrary.org/obo/GAZ_00047020"/>
        <oboInOwl:hasOBONamespace>GAZ</oboInOwl:hasOBONamespace>
        <oboInOwl:id>GAZ:00047037</oboInOwl:id>
        <rdfs:label>Big Moggy Island</rdfs:label>
    </owl:NamedIndividual>
    


    <!-- http://purl.obolibrary.org/obo/GAZ_00047038 -->

    <owl:NamedIndividual rdf:about="http://purl.obolibrary.org/obo/GAZ_00047038">
        <obo:RO_0001025 rdf:resource="http://purl.obolibrary.org/obo/GAZ_00004768"/>
        <obo:IAO_0000115>An island lies 2.5 km off the coast of Otago, within the boundaries of the city of Dunedin.</obo:IAO_0000115>
        <oboInOwl:hasOBONamespace>GAZ</oboInOwl:hasOBONamespace>
        <oboInOwl:id>GAZ:00047038</oboInOwl:id>
        <rdfs:label>White Island</rdfs:label>
    </owl:NamedIndividual>
    


    <!-- http://purl.obolibrary.org/obo/GAZ_00047041 -->

    <owl:NamedIndividual rdf:about="http://purl.obolibrary.org/obo/GAZ_00047041">
        <obo:RO_0001025 rdf:resource="http://purl.obolibrary.org/obo/GAZ_00047047"/>
        <obo:IAO_0000115>A lake in the South Island of New Zealand. Lake Manapouri has four arms, North, South, West and Hope, and some 33 islands, 22 of which are wooded. The Waiau River is its natural outlet.</obo:IAO_0000115>
        <oboInOwl:hasOBONamespace>GAZ</oboInOwl:hasOBONamespace>
        <oboInOwl:id>GAZ:00047041</oboInOwl:id>
        <rdfs:label>Lake Manapouri</rdfs:label>
    </owl:NamedIndividual>
    


    <!-- http://purl.obolibrary.org/obo/GAZ_00047042 -->

    <owl:NamedIndividual rdf:about="http://purl.obolibrary.org/obo/GAZ_00047042">
        <obo:RO_0001025 rdf:resource="http://purl.obolibrary.org/obo/GAZ_00047041"/>
        <oboInOwl:hasOBONamespace>GAZ</oboInOwl:hasOBONamespace>
        <oboInOwl:id>GAZ:00047042</oboInOwl:id>
        <rdfs:label>Channel Islands</rdfs:label>
    </owl:NamedIndividual>
    


    <!-- http://purl.obolibrary.org/obo/GAZ_00047043 -->

    <owl:NamedIndividual rdf:about="http://purl.obolibrary.org/obo/GAZ_00047043">
        <obo:RO_0001025 rdf:resource="http://purl.obolibrary.org/obo/GAZ_00047041"/>
        <oboInOwl:hasOBONamespace>GAZ</oboInOwl:hasOBONamespace>
        <oboInOwl:id>GAZ:00047043</oboInOwl:id>
        <rdfs:label>Rona Island</rdfs:label>
    </owl:NamedIndividual>
    


    <!-- http://purl.obolibrary.org/obo/GAZ_00047044 -->

    <owl:NamedIndividual rdf:about="http://purl.obolibrary.org/obo/GAZ_00047044">
        <obo:RO_0001025 rdf:resource="http://purl.obolibrary.org/obo/GAZ_00047041"/>
        <obo:IAO_0000115>The largest island within Lake Manapouri, in Fiordland National Park, in New Zealand&apos;s South Island. It is one of the largest islands to be found within any New Zealand lake.</obo:IAO_0000115>
        <oboInOwl:hasOBONamespace>GAZ</oboInOwl:hasOBONamespace>
        <oboInOwl:id>GAZ:00047044</oboInOwl:id>
        <rdfs:label>Pomona Island</rdfs:label>
    </owl:NamedIndividual>
    


    <!-- http://purl.obolibrary.org/obo/GAZ_00047045 -->

    <owl:NamedIndividual rdf:about="http://purl.obolibrary.org/obo/GAZ_00047045">
        <obo:RO_0001025 rdf:resource="http://purl.obolibrary.org/obo/GAZ_00047047"/>
        <obo:IAO_0000115>A lake in the south-western corner of the South Island of New Zealand. Several rivers feed the lake, of which the most important is the Eglinton River, which joins the lake from the east, opposite the entrance to North Fiord. The outflow is the Waiau River, which flows south for several km into Lake Manapouri. The town of Te Anau lies at the south-eastern corner of the lake, close to the outflow. Most of the lake is within Fiordland National Park and the Te Wahipounamu World Heritage site.</obo:IAO_0000115>
        <oboInOwl:hasOBONamespace>GAZ</oboInOwl:hasOBONamespace>
        <oboInOwl:id>GAZ:00047045</oboInOwl:id>
        <rdfs:label>Lake Te Anau</rdfs:label>
    </owl:NamedIndividual>
    


    <!-- http://purl.obolibrary.org/obo/GAZ_00047046 -->

    <owl:NamedIndividual rdf:about="http://purl.obolibrary.org/obo/GAZ_00047046">
        <obo:RO_0001025 rdf:resource="http://purl.obolibrary.org/obo/GAZ_00047045"/>
        <oboInOwl:hasOBONamespace>GAZ</oboInOwl:hasOBONamespace>
        <oboInOwl:id>GAZ:00047046</oboInOwl:id>
        <rdfs:label>Entrance Island</rdfs:label>
    </owl:NamedIndividual>
    


    <!-- http://purl.obolibrary.org/obo/GAZ_00047047 -->

    <owl:NamedIndividual rdf:about="http://purl.obolibrary.org/obo/GAZ_00047047">
        <obo:RO_0001025 rdf:resource="http://purl.obolibrary.org/obo/GAZ_00058654"/>
        <obo:IAO_0000115>A national park in the southwest corner of the South Island of New Zealand.</obo:IAO_0000115>
        <oboInOwl:hasOBONamespace>GAZ</oboInOwl:hasOBONamespace>
        <oboInOwl:id>GAZ:00047047</oboInOwl:id>
        <rdfs:label>Fiordland National Park</rdfs:label>
    </owl:NamedIndividual>
    


    <!-- http://purl.obolibrary.org/obo/GAZ_00047048 -->

    <owl:NamedIndividual rdf:about="http://purl.obolibrary.org/obo/GAZ_00047048">
        <obo:RO_0001025 rdf:resource="http://purl.obolibrary.org/obo/GAZ_00047045"/>
        <oboInOwl:hasOBONamespace>GAZ</oboInOwl:hasOBONamespace>
        <oboInOwl:id>GAZ:00047048</oboInOwl:id>
        <rdfs:label>Dome Islands</rdfs:label>
    </owl:NamedIndividual>
    


    <!-- http://purl.obolibrary.org/obo/GAZ_00047050 -->

    <owl:NamedIndividual rdf:about="http://purl.obolibrary.org/obo/GAZ_00047050">
        <obo:RO_0001025 rdf:resource="http://purl.obolibrary.org/obo/GAZ_00030196"/>
        <oboInOwl:hasOBONamespace>GAZ</oboInOwl:hasOBONamespace>
        <oboInOwl:id>GAZ:00047050</oboInOwl:id>
        <rdfs:label>Harwich Island</rdfs:label>
    </owl:NamedIndividual>
    


    <!-- http://purl.obolibrary.org/obo/GAZ_00047051 -->

    <owl:NamedIndividual rdf:about="http://purl.obolibrary.org/obo/GAZ_00047051">
        <obo:RO_0001025 rdf:resource="http://purl.obolibrary.org/obo/GAZ_00011683"/>
        <obo:IAO_0000115>An island located in Lake Rotorua in New Zealand. It has an area of 1.35 km2. The island is a rhyolite lava dome, rising to 180 m above the lake surface. The foreshores of the island also have geothermal springs with hot spring water forming the Hinemoa pool known to locals as Waikimihia.</obo:IAO_0000115>
        <oboInOwl:hasOBONamespace>GAZ</oboInOwl:hasOBONamespace>
        <oboInOwl:id>GAZ:00047051</oboInOwl:id>
        <rdfs:label>Mokoia Island</rdfs:label>
    </owl:NamedIndividual>
    


    <!-- http://purl.obolibrary.org/obo/GAZ_00047052 -->

    <owl:NamedIndividual rdf:about="http://purl.obolibrary.org/obo/GAZ_00047052">
        <obo:RO_0001025 rdf:resource="http://purl.obolibrary.org/obo/GAZ_00047054"/>
        <obo:IAO_0000115>The largest of three roughly parallel lakes running north-south along the northern edge of the Mackenzie Basin in the South Island of New Zealand. It covers an area of 83 km2 and is at an altitude of 700 m above sea level. The lake is fed at its northern end by the braided Godley River, which has its source in the Southern Alps, to the north.</obo:IAO_0000115>
        <oboInOwl:hasOBONamespace>GAZ</oboInOwl:hasOBONamespace>
        <oboInOwl:id>GAZ:00047052</oboInOwl:id>
        <rdfs:label>Lake Tekapo</rdfs:label>
    </owl:NamedIndividual>
    


    <!-- http://purl.obolibrary.org/obo/GAZ_00047053 -->

    <owl:NamedIndividual rdf:about="http://purl.obolibrary.org/obo/GAZ_00047053">
        <obo:RO_0001025 rdf:resource="http://purl.obolibrary.org/obo/GAZ_00047052"/>
        <oboInOwl:hasOBONamespace>GAZ</oboInOwl:hasOBONamespace>
        <oboInOwl:id>GAZ:00047053</oboInOwl:id>
        <rdfs:label>Motuariki Island</rdfs:label>
    </owl:NamedIndividual>
    


    <!-- http://purl.obolibrary.org/obo/GAZ_00047054 -->

    <owl:NamedIndividual rdf:about="http://purl.obolibrary.org/obo/GAZ_00047054">
        <obo:RO_0001025 rdf:resource="http://purl.obolibrary.org/obo/GAZ_00029962"/>
        <obo:IAO_0000115>An elliptical intermontane basin, located in the Mackenzie District, near the centre of the South Island of New Zealand. The majority of the Mackenzie Basin is within Canterbury, although the small part of the basin to the south of the Waitaki River is in Otago.</obo:IAO_0000115>
        <oboInOwl:hasOBONamespace>GAZ</oboInOwl:hasOBONamespace>
        <oboInOwl:id>GAZ:00047054</oboInOwl:id>
        <rdfs:label>Mackenzie Basin</rdfs:label>
    </owl:NamedIndividual>
    


    <!-- http://purl.obolibrary.org/obo/GAZ_00047055 -->

    <owl:NamedIndividual rdf:about="http://purl.obolibrary.org/obo/GAZ_00047055">
        <obo:RO_0001025 rdf:resource="http://purl.obolibrary.org/obo/GAZ_00047054"/>
        <obo:IAO_0000115>An elliptical intermontane basin, located in the Mackenzie District, near the centre of the South Island of New Zealand.</obo:IAO_0000115>
        <oboInOwl:hasOBONamespace>GAZ</oboInOwl:hasOBONamespace>
        <oboInOwl:id>GAZ:00047055</oboInOwl:id>
        <rdfs:label>Lake Pukaki</rdfs:label>
    </owl:NamedIndividual>
    


    <!-- http://purl.obolibrary.org/obo/GAZ_00047056 -->

    <owl:NamedIndividual rdf:about="http://purl.obolibrary.org/obo/GAZ_00047056">
        <obo:RO_0001025 rdf:resource="http://purl.obolibrary.org/obo/GAZ_00047054"/>
        <obo:IAO_0000115>A glacial lake in the Mackenzie Basin of New Zealand&apos;s South Island. It is fed by the Hopkins and Dobson rivers, which have their headwaters in the Southern Alps, and has its outflow in the Ohau River, which itself feeds into the Waitaki River hydroelectric project.</obo:IAO_0000115>
        <oboInOwl:hasOBONamespace>GAZ</oboInOwl:hasOBONamespace>
        <oboInOwl:id>GAZ:00047056</oboInOwl:id>
        <rdfs:label>Lake Ohau</rdfs:label>
    </owl:NamedIndividual>
    


    <!-- http://purl.obolibrary.org/obo/GAZ_00047057 -->

    <owl:NamedIndividual rdf:about="http://purl.obolibrary.org/obo/GAZ_00047057">
        <obo:RO_0001025 rdf:resource="http://purl.obolibrary.org/obo/GAZ_00051946"/>
        <obo:IAO_0000115>An oligotrophic monomictic crater lake situated in the North Island of New Zealand. It has a perimeter of approximately 193 km, a deepest point of 186 m and a surface area of 616 km2. The largest lake by surface area in the country, it is drained by the Waikato River, while its main tributaries are the Waitahanui River, the Tongariro River, and the Taupo-Tauranga River.</obo:IAO_0000115>
        <oboInOwl:hasOBONamespace>GAZ</oboInOwl:hasOBONamespace>
        <oboInOwl:id>GAZ:00047057</oboInOwl:id>
        <rdfs:label>Lake Taupo</rdfs:label>
    </owl:NamedIndividual>
    


    <!-- http://purl.obolibrary.org/obo/GAZ_00047058 -->

    <owl:NamedIndividual rdf:about="http://purl.obolibrary.org/obo/GAZ_00047058">
        <obo:RO_0001025 rdf:resource="http://purl.obolibrary.org/obo/GAZ_00047057"/>
        <oboInOwl:hasOBONamespace>GAZ</oboInOwl:hasOBONamespace>
        <oboInOwl:id>GAZ:00047058</oboInOwl:id>
        <rdfs:label>Motutaiko Island</rdfs:label>
    </owl:NamedIndividual>
    


    <!-- http://purl.obolibrary.org/obo/GAZ_00047059 -->

    <owl:NamedIndividual rdf:about="http://purl.obolibrary.org/obo/GAZ_00047059">
        <obo:RO_0001025 rdf:resource="http://purl.obolibrary.org/obo/GAZ_00004767"/>
        <obo:IAO_0000115>An inland lake (finger lake) in the South Island of New Zealand. It is at in the southwest corner of Otago, near its boundary with Southland. The Dart River flows into the northern end of the lake. The lake is drained by the Kawarau River, which flows out from the lake&apos;s Frankton Arm, 8km east of Queenstown.</obo:IAO_0000115>
        <oboInOwl:hasOBONamespace>GAZ</oboInOwl:hasOBONamespace>
        <oboInOwl:id>GAZ:00047059</oboInOwl:id>
        <rdfs:label>Lake Wakatipu</rdfs:label>
    </owl:NamedIndividual>
    


    <!-- http://purl.obolibrary.org/obo/GAZ_00047060 -->

    <owl:NamedIndividual rdf:about="http://purl.obolibrary.org/obo/GAZ_00047060">
        <obo:RO_0001025 rdf:resource="http://purl.obolibrary.org/obo/GAZ_00047059"/>
        <oboInOwl:hasOBONamespace>GAZ</oboInOwl:hasOBONamespace>
        <oboInOwl:id>GAZ:00047060</oboInOwl:id>
        <rdfs:label>Pigeon Island</rdfs:label>
    </owl:NamedIndividual>
    


    <!-- http://purl.obolibrary.org/obo/GAZ_00047061 -->

    <owl:NamedIndividual rdf:about="http://purl.obolibrary.org/obo/GAZ_00047061">
        <obo:RO_0001025 rdf:resource="http://purl.obolibrary.org/obo/GAZ_00047059"/>
        <oboInOwl:hasOBONamespace>GAZ</oboInOwl:hasOBONamespace>
        <oboInOwl:id>GAZ:00047061</oboInOwl:id>
        <rdfs:label>Pig Island</rdfs:label>
    </owl:NamedIndividual>
    


    <!-- http://purl.obolibrary.org/obo/GAZ_00047062 -->

    <owl:NamedIndividual rdf:about="http://purl.obolibrary.org/obo/GAZ_00047062">
        <obo:RO_0001025 rdf:resource="http://purl.obolibrary.org/obo/GAZ_00004764"/>
        <obo:IAO_0000115>A river that flows south-southeast for 340 km through Central and South Otago to the Pacific Ocean, 75 km south west of Dunedin.</obo:IAO_0000115>
        <oboInOwl:hasOBONamespace>GAZ</oboInOwl:hasOBONamespace>
        <oboInOwl:id>GAZ:00047062</oboInOwl:id>
        <rdfs:label>Clutha River</rdfs:label>
    </owl:NamedIndividual>
    


    <!-- http://purl.obolibrary.org/obo/GAZ_00047063 -->

    <owl:NamedIndividual rdf:about="http://purl.obolibrary.org/obo/GAZ_00047063">
        <obo:RO_0001025 rdf:resource="http://purl.obolibrary.org/obo/GAZ_00047062"/>
        <oboInOwl:hasOBONamespace>GAZ</oboInOwl:hasOBONamespace>
        <oboInOwl:id>GAZ:00047063</oboInOwl:id>
        <rdfs:label>Clutha River Delta</rdfs:label>
    </owl:NamedIndividual>
    


    <!-- http://purl.obolibrary.org/obo/GAZ_00047064 -->

    <owl:NamedIndividual rdf:about="http://purl.obolibrary.org/obo/GAZ_00047064">
        <obo:RO_0001025 rdf:resource="http://purl.obolibrary.org/obo/GAZ_00047063"/>
        <obo:IAO_0000115>A large, flat island sitting in the delta of the Clutha River in the South Island of New Zealand, downstream from the town of Balclutha.</obo:IAO_0000115>
        <oboInOwl:hasOBONamespace>GAZ</oboInOwl:hasOBONamespace>
        <oboInOwl:id>GAZ:00047064</oboInOwl:id>
        <rdfs:label>Inch Clutha</rdfs:label>
    </owl:NamedIndividual>
    


    <!-- http://purl.obolibrary.org/obo/GAZ_00047065 -->

    <owl:NamedIndividual rdf:about="http://purl.obolibrary.org/obo/GAZ_00047065">
        <obo:RO_0001025 rdf:resource="http://purl.obolibrary.org/obo/GAZ_00004764"/>
        <oboInOwl:hasOBONamespace>GAZ</oboInOwl:hasOBONamespace>
        <oboInOwl:id>GAZ:00047065</oboInOwl:id>
        <rdfs:label>Rakaia River</rdfs:label>
    </owl:NamedIndividual>
    


    <!-- http://purl.obolibrary.org/obo/GAZ_00047066 -->

    <owl:NamedIndividual rdf:about="http://purl.obolibrary.org/obo/GAZ_00047066">
        <obo:RO_0001025 rdf:resource="http://purl.obolibrary.org/obo/GAZ_00047065"/>
        <oboInOwl:hasOBONamespace>GAZ</oboInOwl:hasOBONamespace>
        <oboInOwl:id>GAZ:00047066</oboInOwl:id>
        <rdfs:label>Rakaia River delta</rdfs:label>
    </owl:NamedIndividual>
    


    <!-- http://purl.obolibrary.org/obo/GAZ_00047067 -->

    <owl:NamedIndividual rdf:about="http://purl.obolibrary.org/obo/GAZ_00047067">
        <obo:RO_0001025 rdf:resource="http://purl.obolibrary.org/obo/GAZ_00047066"/>
        <oboInOwl:hasOBONamespace>GAZ</oboInOwl:hasOBONamespace>
        <oboInOwl:id>GAZ:00047067</oboInOwl:id>
        <rdfs:label>Rakaia Island</rdfs:label>
    </owl:NamedIndividual>
    


    <!-- http://purl.obolibrary.org/obo/GAZ_00047068 -->

    <owl:NamedIndividual rdf:about="http://purl.obolibrary.org/obo/GAZ_00047068">
        <obo:RO_0001025 rdf:resource="http://purl.obolibrary.org/obo/GAZ_00004764"/>
        <oboInOwl:hasOBONamespace>GAZ</oboInOwl:hasOBONamespace>
        <oboInOwl:id>GAZ:00047068</oboInOwl:id>
        <rdfs:label>Rangitata River</rdfs:label>
    </owl:NamedIndividual>
    


    <!-- http://purl.obolibrary.org/obo/GAZ_00047069 -->

    <owl:NamedIndividual rdf:about="http://purl.obolibrary.org/obo/GAZ_00047069">
        <obo:RO_0001025 rdf:resource="http://purl.obolibrary.org/obo/GAZ_00047068"/>
        <oboInOwl:hasOBONamespace>GAZ</oboInOwl:hasOBONamespace>
        <oboInOwl:id>GAZ:00047069</oboInOwl:id>
        <rdfs:label>Rangitata River delta</rdfs:label>
    </owl:NamedIndividual>
    


    <!-- http://purl.obolibrary.org/obo/GAZ_00047070 -->

    <owl:NamedIndividual rdf:about="http://purl.obolibrary.org/obo/GAZ_00047070">
        <obo:RO_0001025 rdf:resource="http://purl.obolibrary.org/obo/GAZ_00047069"/>
        <oboInOwl:hasOBONamespace>GAZ</oboInOwl:hasOBONamespace>
        <oboInOwl:id>GAZ:00047070</oboInOwl:id>
        <rdfs:label>Rangitata Island</rdfs:label>
    </owl:NamedIndividual>
    


    <!-- http://purl.obolibrary.org/obo/GAZ_00047071 -->

    <owl:NamedIndividual rdf:about="http://purl.obolibrary.org/obo/GAZ_00047071">
        <obo:RO_0001025 rdf:resource="http://purl.obolibrary.org/obo/GAZ_00007139"/>
        <obo:IAO_0000115>A rock located 8 km NWW of L&apos;Esperance Rock.</obo:IAO_0000115>
        <oboInOwl:hasOBONamespace>GAZ</oboInOwl:hasOBONamespace>
        <oboInOwl:id>GAZ:00047071</oboInOwl:id>
        <rdfs:label>L&apos;Havre Rock</rdfs:label>
    </owl:NamedIndividual>
    


    <!-- http://purl.obolibrary.org/obo/GAZ_00047072 -->

    <owl:NamedIndividual rdf:about="http://purl.obolibrary.org/obo/GAZ_00047072">
        <obo:RO_0001025 rdf:resource="http://purl.obolibrary.org/obo/GAZ_00007139"/>
        <obo:IAO_0000115>A rock located about 4 km north of Macauley Island.</obo:IAO_0000115>
        <oboInOwl:hasOBONamespace>GAZ</oboInOwl:hasOBONamespace>
        <oboInOwl:id>GAZ:00047072</oboInOwl:id>
        <rdfs:label>Macdonald Rock</rdfs:label>
    </owl:NamedIndividual>
    


    <!-- http://purl.obolibrary.org/obo/GAZ_00047073 -->

    <owl:NamedIndividual rdf:about="http://purl.obolibrary.org/obo/GAZ_00047073">
        <obo:RO_0001025 rdf:resource="http://purl.obolibrary.org/obo/GAZ_00007139"/>
        <obo:IAO_0000115>An island located adjecent to Macauley Island.</obo:IAO_0000115>
        <oboInOwl:hasOBONamespace>GAZ</oboInOwl:hasOBONamespace>
        <oboInOwl:id>GAZ:00047073</oboInOwl:id>
        <rdfs:label>Haszard Island</rdfs:label>
    </owl:NamedIndividual>
    


    <!-- http://purl.obolibrary.org/obo/GAZ_00047074 -->

    <owl:NamedIndividual rdf:about="http://purl.obolibrary.org/obo/GAZ_00047074">
        <obo:RO_0001025 rdf:resource="http://purl.obolibrary.org/obo/GAZ_00007139"/>
        <obo:IAO_0000115>With nearby Curtis island, the uplifted portion of a submarine volcano astride the Kermadec Ridge. The age of the small islands is considered to be Pleistocene, and rocks consist dominantly, if not entirely, of andesitic pyroclastic-flow deposits (Lloyd, 1992). Curtis Island, only 500 x 800 m in diameter and 137-m high, contains a large, fumarolically active crater whose floor is only 10 m above sea level. Reports of possible historical eruptions probably represent increased thermal activity. Geologic studies have documented a remarkable uplift of 18 m of Curtis Island during the past 200 years, with 7 m of uplift occurring between 1929 and 1964 (Doyle et al., 1979). An active submarine magmatic or solfataric vent is believed to exist near Curtis Island, but its activity cannot unequivocally be associated with Curtis volcano (Lloyd, 1992).</obo:IAO_0000115>
        <oboInOwl:hasOBONamespace>GAZ</oboInOwl:hasOBONamespace>
        <oboInOwl:id>GAZ:00047074</oboInOwl:id>
        <rdfs:label>Cheeseman Island</rdfs:label>
    </owl:NamedIndividual>
    


    <!-- http://purl.obolibrary.org/obo/GAZ_00047075 -->

    <owl:NamedIndividual rdf:about="http://purl.obolibrary.org/obo/GAZ_00047075">
        <obo:RO_0001025 rdf:resource="http://purl.obolibrary.org/obo/GAZ_00007139"/>
        <obo:IAO_0000115>A bank located 103 km SSW of L&apos;Esperance Rock, with a least depth of 48 meters.</obo:IAO_0000115>
        <oboInOwl:hasOBONamespace>GAZ</oboInOwl:hasOBONamespace>
        <oboInOwl:id>GAZ:00047075</oboInOwl:id>
        <rdfs:label>Star of Bengal Bank</rdfs:label>
    </owl:NamedIndividual>
    


    <!-- http://purl.obolibrary.org/obo/GAZ_00050840 -->

    <owl:NamedIndividual rdf:about="http://purl.obolibrary.org/obo/GAZ_00050840">
        <obo:RO_0001025 rdf:resource="http://purl.obolibrary.org/obo/GAZ_00017424"/>
        <obo:IAO_0000115>A rock in the Main Group of the Bounty Islands.</obo:IAO_0000115>
        <oboInOwl:hasOBONamespace>GAZ</oboInOwl:hasOBONamespace>
        <oboInOwl:id>GAZ:00050840</oboInOwl:id>
        <rdfs:label>Skua Rock</rdfs:label>
    </owl:NamedIndividual>
    


    <!-- http://purl.obolibrary.org/obo/GAZ_00051944 -->

    <owl:NamedIndividual rdf:about="http://purl.obolibrary.org/obo/GAZ_00051944">
        <obo:RO_0001025 rdf:resource="http://purl.obolibrary.org/obo/GAZ_00009535"/>
        <obo:RO_0001025 rdf:resource="http://purl.obolibrary.org/obo/GAZ_00051945"/>
        <obo:IAO_0000115>The NW-most caldera of the Taupo volcanic zone. Rotorua is the only single-event caldera in the Taupo volcanic zone and was formed about 220,000 years ago following eruption of the &gt;340 cu km rhyolitic Mamaku Ignimbrite. Although caldera collapse occurred in a single event, the process was complex and involved multiple collapse blocks. The major city of Rotorua lies at the south end of the lake that fills much of the caldera. Post-collapse eruptive activity, which ceased during the Pleistocene, has been restricted to lava dome extrusion without major explosive activity. The youngest eruptive activity at Rotorua consisted of the eruption of three lava domes less than 25,000 years ago. The major thermal areas of Takeke, Tikitere, Lake Rotokawa, and Rotorua-Whakarewarewa are located within the caldera or outside its rim, and the city of Rotorua lies within and adjacent to active geothermal fields.</obo:IAO_0000115>
        <oboInOwl:hasOBONamespace>GAZ</oboInOwl:hasOBONamespace>
        <oboInOwl:id>GAZ:00051944</oboInOwl:id>
        <rdfs:label>Rotorua Caldera</rdfs:label>
    </owl:NamedIndividual>
    


    <!-- http://purl.obolibrary.org/obo/GAZ_00051945 -->

    <owl:NamedIndividual rdf:about="http://purl.obolibrary.org/obo/GAZ_00051945">
        <obo:RO_0001025 rdf:resource="http://purl.obolibrary.org/obo/GAZ_00004765"/>
        <obo:IAO_0000115>An active volcanic area in the North Island of New Zealand.</obo:IAO_0000115>
        <oboInOwl:hasOBONamespace>GAZ</oboInOwl:hasOBONamespace>
        <oboInOwl:id>GAZ:00051945</oboInOwl:id>
        <rdfs:label>Taupo Volcanic Zone</rdfs:label>
    </owl:NamedIndividual>
    


    <!-- http://purl.obolibrary.org/obo/GAZ_00051946 -->

    <owl:NamedIndividual rdf:about="http://purl.obolibrary.org/obo/GAZ_00051946">
        <obo:RO_0001025 rdf:resource="http://purl.obolibrary.org/obo/GAZ_00051945"/>
        <obo:IAO_0000115>A rhyolitic volcano of the Taupo volcanic zone, is a large, roughly 35 km wide caldera with poorly defined margins. It is a type example of an &quot;inverse volcano&quot; that slopes inward towards the most recent vent location. The Taupo caldera, now filled by Lake Taupo, largely formed as a result of the voluminous eruption of the Oruanui Tephra about 22,600 years before present (BP). This was the largest known eruption at Taupo, producing about 1170 cu km of tephra. This eruption was preceded during the late Pleistocene by the eruption of a large number of rhyolitic lava domes north of Lake Taupo. Large explosive eruptions have occurred frequently during the Holocene from many vents within Lake Taupo and near its margins. The most recent major eruption took place about 1800 years BP from at least three vents along a NE-SW-trending fissure centered on the Horomotangi Reefs. This extremely violent eruption was New Zealand&apos;s largest during the Holocene and produced the thin but widespread phreatoplinian Taupo Ignimbrite, which covered 20,000 km2 of North Island.</obo:IAO_0000115>
        <oboInOwl:hasOBONamespace>GAZ</oboInOwl:hasOBONamespace>
        <oboInOwl:id>GAZ:00051946</oboInOwl:id>
        <rdfs:label>Taupo Caldera</rdfs:label>
    </owl:NamedIndividual>
    


    <!-- http://purl.obolibrary.org/obo/GAZ_00053293 -->

    <owl:NamedIndividual rdf:about="http://purl.obolibrary.org/obo/GAZ_00053293">
        <obo:RO_0001025 rdf:resource="http://purl.obolibrary.org/obo/GAZ_00051945"/>
        <obo:IAO_0000115>An active stratovolcano at the southern end of the Taupo Volcanic Zone in New Zealand. It is 23 km northeast of Ohakune and 40 km southwest of the southern shore of Lake Taupo, within Tongariro National Park.</obo:IAO_0000115>
        <oboInOwl:hasOBONamespace>GAZ</oboInOwl:hasOBONamespace>
        <oboInOwl:id>GAZ:00053293</oboInOwl:id>
        <rdfs:label>Mount Ruapehu</rdfs:label>
    </owl:NamedIndividual>
    


    <!-- http://purl.obolibrary.org/obo/GAZ_00053294 -->

    <owl:NamedIndividual rdf:about="http://purl.obolibrary.org/obo/GAZ_00053294">
        <obo:RO_0001025 rdf:resource="http://purl.obolibrary.org/obo/GAZ_00051945"/>
        <obo:IAO_0000115>An active stratovolcano in New Zealand. It is the youngest vent and highest peak in the Tongariro volcanic complex on the Central Plateau of the North Island.</obo:IAO_0000115>
        <oboInOwl:hasOBONamespace>GAZ</oboInOwl:hasOBONamespace>
        <oboInOwl:id>GAZ:00053294</oboInOwl:id>
        <rdfs:label>Mount Ngauruhoe</rdfs:label>
    </owl:NamedIndividual>
    


    <!-- http://purl.obolibrary.org/obo/GAZ_00053295 -->

    <owl:NamedIndividual rdf:about="http://purl.obolibrary.org/obo/GAZ_00053295">
        <obo:RO_0001025 rdf:resource="http://purl.obolibrary.org/obo/GAZ_00051945"/>
        <obo:RO_0001025 rdf:resource="http://purl.obolibrary.org/obo/GAZ_00053847"/>
        <obo:IAO_0000115>A volcanic mountain 24.1 km southeast of Rotorua in the North Island of New Zealand. It consists of a series of rhyolitic lava domes that were fissured down the middle by a basaltic eruption in 1886. The peaks are Ruawahia Peak, Tarawera Peak and Wahanga Peak.</obo:IAO_0000115>
        <oboInOwl:hasOBONamespace>GAZ</oboInOwl:hasOBONamespace>
        <oboInOwl:id>GAZ:00053295</oboInOwl:id>
        <rdfs:label>Mount Tarawera</rdfs:label>
    </owl:NamedIndividual>
    


    <!-- http://purl.obolibrary.org/obo/GAZ_00053808 -->

    <owl:NamedIndividual rdf:about="http://purl.obolibrary.org/obo/GAZ_00053808">
        <obo:RO_0001025 rdf:resource="http://purl.obolibrary.org/obo/GAZ_00007139"/>
        <obo:IAO_0000115>Twin submarine volcanoes, known informally as Volcano W, were discovered during a New Zealand-American submarine vent mapping expedition to the Kermadec arc in 2004. The two deep-water basaltic volcanoes lie SW of Curtis Island. The summits of both volcanoes are cut by small calderas, and evidence of diffuse hydrothermal venting was observed on the SE volcano in 2005. The SE volcano rises to within about 900 m of the sea surface and contains a cone in its summit caldera. The caldera walls expose pillow lavas, pillow tubes, localized sheet flows, and pillow breccias, with higher proportions of volcaniclastic breccias in the upper portion.</obo:IAO_0000115>
        <oboInOwl:hasOBONamespace>GAZ</oboInOwl:hasOBONamespace>
        <oboInOwl:id>GAZ:00053808</oboInOwl:id>
        <rdfs:label>Volcano W</rdfs:label>
    </owl:NamedIndividual>
    


    <!-- http://purl.obolibrary.org/obo/GAZ_00053809 -->

    <owl:NamedIndividual rdf:about="http://purl.obolibrary.org/obo/GAZ_00053809">
        <obo:RO_0001025 rdf:resource="http://purl.obolibrary.org/obo/GAZ_00007139"/>
        <obo:IAO_0000115>A submarine volcano. The flat summit of the basaltic-to-dacitic volcano is cut by a 700-m-wide crater containing a central cone. The volcano reaches to within 65 m of the sea surface, and the summit is cut by numerous small explosion pits and craters. Much of the edifice is blanketed by dacitic pumice, and several edifice-collapse scarps cut its flanks. Large satellite cones are found on the ENE and SSW flanks, and a chain of eight small satellitic cones that fed recent andesitic-dacitic lava flows lies on the west flank. A large hydrothermal vent field was found within the summit crater.</obo:IAO_0000115>
        <oboInOwl:hasOBONamespace>GAZ</oboInOwl:hasOBONamespace>
        <oboInOwl:id>GAZ:00053809</oboInOwl:id>
        <rdfs:label>Giggenbach Seamount</rdfs:label>
    </owl:NamedIndividual>
    


    <!-- http://purl.obolibrary.org/obo/GAZ_00053810 -->

    <owl:NamedIndividual rdf:about="http://purl.obolibrary.org/obo/GAZ_00053810">
        <obo:RO_0001025 rdf:resource="http://purl.obolibrary.org/obo/GAZ_00007139"/>
        <obo:IAO_0000115>A seamount (submarine volcano) that rises to within 100 m of the sea surface about halfway between the Kermadec and Tonga island groups. The volcano lies at the southern end of the Tonga Ridge and is slightly offset from the Kermadec volcanoes. Small parasitic cones occur on the north and west flanks of the basaltic submarine volcano, which rises from a depth of about 1500 m and was named for one of the New Zealand Navy bathymetric survey ships that documented its morphology. A large 8 x 13 km wide submarine caldera with a depth of more than 1500 m lies to the NNE. Numerous eruptions from Monowai have been detected from submarine acoustic signals since it was first recognized as a volcano in 1977.</obo:IAO_0000115>
        <oboInOwl:hasOBONamespace>GAZ</oboInOwl:hasOBONamespace>
        <oboInOwl:id>GAZ:00053810</oboInOwl:id>
        <rdfs:label>Monowai Seamount</rdfs:label>
    </owl:NamedIndividual>
    


    <!-- http://purl.obolibrary.org/obo/GAZ_00053811 -->

    <owl:NamedIndividual rdf:about="http://purl.obolibrary.org/obo/GAZ_00053811">
        <obo:RO_0001025 rdf:resource="http://purl.obolibrary.org/obo/GAZ_00007143"/>
        <obo:IAO_0000115>A caldera formed during a major dacitic explosive eruption about 2200 years ago, truncated the western side of the island and is 6.5 x 4 km wide. Its long axis is parallel to the tectonic fabric of the Havre Trough that lies west of the volcanic arc.</obo:IAO_0000115>
        <oboInOwl:hasOBONamespace>GAZ</oboInOwl:hasOBONamespace>
        <oboInOwl:id>GAZ:00053811</oboInOwl:id>
        <rdfs:label>Denham Caldera</rdfs:label>
    </owl:NamedIndividual>
    


    <!-- http://purl.obolibrary.org/obo/GAZ_00053812 -->

    <owl:NamedIndividual rdf:about="http://purl.obolibrary.org/obo/GAZ_00053812">
        <obo:RO_0001025 rdf:resource="http://purl.obolibrary.org/obo/GAZ_00142240"/>
        <obo:IAO_0000115>A crater lake.</obo:IAO_0000115>
        <oboInOwl:hasOBONamespace>GAZ</oboInOwl:hasOBONamespace>
        <oboInOwl:id>GAZ:00053812</oboInOwl:id>
        <rdfs:label>Blue Lake</rdfs:label>
    </owl:NamedIndividual>
    


    <!-- http://purl.obolibrary.org/obo/GAZ_00053813 -->

    <owl:NamedIndividual rdf:about="http://purl.obolibrary.org/obo/GAZ_00053813">
        <obo:RO_0001025 rdf:resource="http://purl.obolibrary.org/obo/GAZ_00142240"/>
        <obo:IAO_0000115>A crater (freshwater) lake.</obo:IAO_0000115>
        <oboInOwl:hasOBONamespace>GAZ</oboInOwl:hasOBONamespace>
        <oboInOwl:id>GAZ:00053813</oboInOwl:id>
        <rdfs:label>Tui Lake</rdfs:label>
    </owl:NamedIndividual>
    


    <!-- http://purl.obolibrary.org/obo/GAZ_00053814 -->

    <owl:NamedIndividual rdf:about="http://purl.obolibrary.org/obo/GAZ_00053814">
        <obo:RO_0001025 rdf:resource="http://purl.obolibrary.org/obo/GAZ_00053816"/>
        <obo:IAO_0000115>Satellite islands NE of Raoul Island to the E of the Meyer Islands.</obo:IAO_0000115>
        <oboInOwl:hasOBONamespace>GAZ</oboInOwl:hasOBONamespace>
        <oboInOwl:id>GAZ:00053814</oboInOwl:id>
        <rdfs:label>Herald Islets</rdfs:label>
    </owl:NamedIndividual>
    


    <!-- http://purl.obolibrary.org/obo/GAZ_00053815 -->

    <owl:NamedIndividual rdf:about="http://purl.obolibrary.org/obo/GAZ_00053815">
        <obo:RO_0001025 rdf:resource="http://purl.obolibrary.org/obo/GAZ_00053816"/>
        <obo:IAO_0000115>Two larger islands, and several very small islands, NE of Raoul Island.</obo:IAO_0000115>
        <oboInOwl:hasOBONamespace>GAZ</oboInOwl:hasOBONamespace>
        <oboInOwl:id>GAZ:00053815</oboInOwl:id>
        <rdfs:label>Meyer Islands</rdfs:label>
    </owl:NamedIndividual>
    


    <!-- http://purl.obolibrary.org/obo/GAZ_00053816 -->

    <owl:NamedIndividual rdf:about="http://purl.obolibrary.org/obo/GAZ_00053816">
        <obo:RO_0001025 rdf:resource="http://purl.obolibrary.org/obo/GAZ_00007139"/>
        <obo:IAO_0000115>An archipelago consisting of Raoul Island and its satellite islands and rocks.</obo:IAO_0000115>
        <oboInOwl:hasOBONamespace>GAZ</oboInOwl:hasOBONamespace>
        <oboInOwl:id>GAZ:00053816</oboInOwl:id>
        <rdfs:label>Raoul Archipelago</rdfs:label>
    </owl:NamedIndividual>
    


    <!-- http://purl.obolibrary.org/obo/GAZ_00053817 -->

    <owl:NamedIndividual rdf:about="http://purl.obolibrary.org/obo/GAZ_00053817">
        <obo:RO_0001025 rdf:resource="http://purl.obolibrary.org/obo/GAZ_00053816"/>
        <obo:IAO_0000115>A satellite island NE of Raoul Island.</obo:IAO_0000115>
        <oboInOwl:hasOBONamespace>GAZ</oboInOwl:hasOBONamespace>
        <oboInOwl:id>GAZ:00053817</oboInOwl:id>
        <rdfs:label>Nugent Island</rdfs:label>
    </owl:NamedIndividual>
    


    <!-- http://purl.obolibrary.org/obo/GAZ_00053818 -->

    <owl:NamedIndividual rdf:about="http://purl.obolibrary.org/obo/GAZ_00053818">
        <obo:RO_0001025 rdf:resource="http://purl.obolibrary.org/obo/GAZ_00053816"/>
        <obo:IAO_0000115>A satellite island NE of Raoul Island, NW of Rayner Rock.</obo:IAO_0000115>
        <oboInOwl:hasOBONamespace>GAZ</oboInOwl:hasOBONamespace>
        <oboInOwl:id>GAZ:00053818</oboInOwl:id>
        <rdfs:label>Fishing Rock</rdfs:label>
    </owl:NamedIndividual>
    


    <!-- http://purl.obolibrary.org/obo/GAZ_00053819 -->

    <owl:NamedIndividual rdf:about="http://purl.obolibrary.org/obo/GAZ_00053819">
        <obo:RO_0001025 rdf:resource="http://purl.obolibrary.org/obo/GAZ_00053816"/>
        <obo:IAO_0000115>A satellite island NE of Raoul Island.</obo:IAO_0000115>
        <oboInOwl:hasOBONamespace>GAZ</oboInOwl:hasOBONamespace>
        <oboInOwl:id>GAZ:00053819</oboInOwl:id>
        <rdfs:label>Napier Island</rdfs:label>
    </owl:NamedIndividual>
    


    <!-- http://purl.obolibrary.org/obo/GAZ_00053820 -->

    <owl:NamedIndividual rdf:about="http://purl.obolibrary.org/obo/GAZ_00053820">
        <obo:RO_0001025 rdf:resource="http://purl.obolibrary.org/obo/GAZ_00053816"/>
        <obo:IAO_0000115>A rock NE of Raoul Island, NE of Rayner Point.</obo:IAO_0000115>
        <oboInOwl:hasOBONamespace>GAZ</oboInOwl:hasOBONamespace>
        <oboInOwl:id>GAZ:00053820</oboInOwl:id>
        <rdfs:label>Egeria Rock</rdfs:label>
    </owl:NamedIndividual>
    


    <!-- http://purl.obolibrary.org/obo/GAZ_00053821 -->

    <owl:NamedIndividual rdf:about="http://purl.obolibrary.org/obo/GAZ_00053821">
        <obo:RO_0001025 rdf:resource="http://purl.obolibrary.org/obo/GAZ_00053815"/>
        <oboInOwl:hasOBONamespace>GAZ</oboInOwl:hasOBONamespace>
        <oboInOwl:id>GAZ:00053821</oboInOwl:id>
        <rdfs:label>South Meyer Island</rdfs:label>
    </owl:NamedIndividual>
    


    <!-- http://purl.obolibrary.org/obo/GAZ_00053822 -->

    <owl:NamedIndividual rdf:about="http://purl.obolibrary.org/obo/GAZ_00053822">
        <obo:RO_0001025 rdf:resource="http://purl.obolibrary.org/obo/GAZ_00053815"/>
        <oboInOwl:hasOBONamespace>GAZ</oboInOwl:hasOBONamespace>
        <oboInOwl:id>GAZ:00053822</oboInOwl:id>
        <rdfs:label>North Meyer Island</rdfs:label>
    </owl:NamedIndividual>
    


    <!-- http://purl.obolibrary.org/obo/GAZ_00053823 -->

    <owl:NamedIndividual rdf:about="http://purl.obolibrary.org/obo/GAZ_00053823">
        <obo:RO_0001025 rdf:resource="http://purl.obolibrary.org/obo/GAZ_00053814"/>
        <obo:IAO_0000115>Satellite islands NE of Raoul Island.</obo:IAO_0000115>
        <oboInOwl:hasOBONamespace>GAZ</oboInOwl:hasOBONamespace>
        <oboInOwl:id>GAZ:00053823</oboInOwl:id>
        <rdfs:label>Chanter Islands</rdfs:label>
    </owl:NamedIndividual>
    


    <!-- http://purl.obolibrary.org/obo/GAZ_00053824 -->

    <owl:NamedIndividual rdf:about="http://purl.obolibrary.org/obo/GAZ_00053824">
        <obo:RO_0001025 rdf:resource="http://purl.obolibrary.org/obo/GAZ_00053814"/>
        <obo:IAO_0000115>A satellite island NE of Raoul Island. The most N of the Herald Islands.</obo:IAO_0000115>
        <oboInOwl:hasOBONamespace>GAZ</oboInOwl:hasOBONamespace>
        <oboInOwl:id>GAZ:00053824</oboInOwl:id>
        <rdfs:label>Dayrell Island</rdfs:label>
    </owl:NamedIndividual>
    


    <!-- http://purl.obolibrary.org/obo/GAZ_00053825 -->

    <owl:NamedIndividual rdf:about="http://purl.obolibrary.org/obo/GAZ_00053825">
        <obo:RO_0001025 rdf:resource="http://purl.obolibrary.org/obo/GAZ_00053823"/>
        <obo:IAO_0000115>A satellite island NE of Raoul Island.</obo:IAO_0000115>
        <oboInOwl:hasOBONamespace>GAZ</oboInOwl:hasOBONamespace>
        <oboInOwl:id>GAZ:00053825</oboInOwl:id>
        <rdfs:label>West Chanter Island</rdfs:label>
    </owl:NamedIndividual>
    


    <!-- http://purl.obolibrary.org/obo/GAZ_00053826 -->

    <owl:NamedIndividual rdf:about="http://purl.obolibrary.org/obo/GAZ_00053826">
        <obo:RO_0001025 rdf:resource="http://purl.obolibrary.org/obo/GAZ_00053823"/>
        <obo:IAO_0000115>A satellite island to the NE of Raoul Island.</obo:IAO_0000115>
        <oboInOwl:hasOBONamespace>GAZ</oboInOwl:hasOBONamespace>
        <oboInOwl:id>GAZ:00053826</oboInOwl:id>
        <rdfs:label>South Chanter Island</rdfs:label>
    </owl:NamedIndividual>
    


    <!-- http://purl.obolibrary.org/obo/GAZ_00053827 -->

    <owl:NamedIndividual rdf:about="http://purl.obolibrary.org/obo/GAZ_00053827">
        <obo:RO_0001025 rdf:resource="http://purl.obolibrary.org/obo/GAZ_00053823"/>
        <obo:IAO_0000115>A satellite island NE of Raoul Island.</obo:IAO_0000115>
        <oboInOwl:hasOBONamespace>GAZ</oboInOwl:hasOBONamespace>
        <oboInOwl:id>GAZ:00053827</oboInOwl:id>
        <rdfs:label>North Chanter Island</rdfs:label>
    </owl:NamedIndividual>
    


    <!-- http://purl.obolibrary.org/obo/GAZ_00053828 -->

    <owl:NamedIndividual rdf:about="http://purl.obolibrary.org/obo/GAZ_00053828">
        <obo:RO_0001025 rdf:resource="http://purl.obolibrary.org/obo/GAZ_00053816"/>
        <obo:IAO_0000115>Satellite rocks located SW of Raoul Island.</obo:IAO_0000115>
        <oboInOwl:hasOBONamespace>GAZ</oboInOwl:hasOBONamespace>
        <oboInOwl:id>GAZ:00053828</oboInOwl:id>
        <rdfs:label>Dougall Rocks</rdfs:label>
    </owl:NamedIndividual>
    


    <!-- http://purl.obolibrary.org/obo/GAZ_00053829 -->

    <owl:NamedIndividual rdf:about="http://purl.obolibrary.org/obo/GAZ_00053829">
        <obo:RO_0001025 rdf:resource="http://purl.obolibrary.org/obo/GAZ_00053816"/>
        <obo:IAO_0000115>Satellite islands located SW of Raoul Island.</obo:IAO_0000115>
        <oboInOwl:hasOBONamespace>GAZ</oboInOwl:hasOBONamespace>
        <oboInOwl:id>GAZ:00053829</oboInOwl:id>
        <rdfs:label>Milne Islands</rdfs:label>
    </owl:NamedIndividual>
    


    <!-- http://purl.obolibrary.org/obo/GAZ_00053832 -->

    <owl:NamedIndividual rdf:about="http://purl.obolibrary.org/obo/GAZ_00053832">
        <obo:RO_0001025 rdf:resource="http://purl.obolibrary.org/obo/GAZ_00053834"/>
        <obo:IAO_0000115>A geothermal area in the North Island of New Zealand. It is situated approximately 5Km east of Kaikohe and is centered around the village of Ngawha Springs.</obo:IAO_0000115>
        <oboInOwl:hasOBONamespace>GAZ</oboInOwl:hasOBONamespace>
        <oboInOwl:id>GAZ:00053832</oboInOwl:id>
        <rdfs:label>Ngawha Geothermal Field</rdfs:label>
    </owl:NamedIndividual>
    


    <!-- http://purl.obolibrary.org/obo/GAZ_00053833 -->

    <owl:NamedIndividual rdf:about="http://purl.obolibrary.org/obo/GAZ_00053833">
        <obo:RO_0001025 rdf:resource="http://purl.obolibrary.org/obo/GAZ_00029928"/>
        <obo:IAO_0000115>A small lake in the Northland Region of New Zealand. It is located just to the north of the town of Kaikohe.</obo:IAO_0000115>
        <oboInOwl:hasOBONamespace>GAZ</oboInOwl:hasOBONamespace>
        <oboInOwl:id>GAZ:00053833</oboInOwl:id>
        <rdfs:label>Lake Omapere</rdfs:label>
    </owl:NamedIndividual>
    


    <!-- http://purl.obolibrary.org/obo/GAZ_00053834 -->

    <owl:NamedIndividual rdf:about="http://purl.obolibrary.org/obo/GAZ_00053834">
        <obo:RO_0001025 rdf:resource="http://purl.obolibrary.org/obo/GAZ_00029928"/>
        <obo:IAO_0000115>A volcanic field at the upper end of the Northland Peninsula contains 30 Pleistocene to upper-Holocene eruptive centers, consisting primarily of basaltic scoria cones, lava flows, and small shield volcanoes, along with minor rhyolitic lava flows and domes. The field lies at the northern end of the Northland Intraplate Province, and volcanism has progressively shifted to the SE, with the younger Taheke Basalts being aligned along a NE trend at the southern end of the volcanic field.</obo:IAO_0000115>
        <oboInOwl:hasOBONamespace>GAZ</oboInOwl:hasOBONamespace>
        <oboInOwl:id>GAZ:00053834</oboInOwl:id>
        <rdfs:label>Kaikohe-Bay of Islands Volcanic Field</rdfs:label>
    </owl:NamedIndividual>
    


    <!-- http://purl.obolibrary.org/obo/GAZ_00053835 -->

    <owl:NamedIndividual rdf:about="http://purl.obolibrary.org/obo/GAZ_00053835">
        <obo:RO_0001025 rdf:resource="http://purl.obolibrary.org/obo/GAZ_00029928"/>
        <obo:IAO_0000115>A volcanic field that consists of Quaternary basaltic scoria cones and lava flows. The field lies in the central part of the Northland Peninsula, at the southernmost end of the Northland Intraplate Province. In addition to the younger dominantly basaltic rocks, Miocene dacitic lava domes and rhyolitic breccias are also present at Whangarei. Quaternary volcanics form a group of large cones SE of Whangarei, a NE-aligned group of scoria cones north of the city, and a group of lava flows east of the city along a major fault.</obo:IAO_0000115>
        <oboInOwl:hasOBONamespace>GAZ</oboInOwl:hasOBONamespace>
        <oboInOwl:id>GAZ:00053835</oboInOwl:id>
        <rdfs:label>Whangarei Volcanic Field</rdfs:label>
    </owl:NamedIndividual>
    


    <!-- http://purl.obolibrary.org/obo/GAZ_00053836 -->

    <owl:NamedIndividual rdf:about="http://purl.obolibrary.org/obo/GAZ_00053836">
        <obo:RO_0001025 rdf:resource="http://purl.obolibrary.org/obo/GAZ_00007139"/>
        <obo:IAO_0000115>A submarine volcano located NE of the Healy submarine volcano, contains an oval-shaped summit caldera 3-3.5 km wide. The volcano is elongated in a NW-SE direction, and the high point of the dominantly dacitic volcano lies on the NW caldera rim at about 1350 m below the sea surface. The caldera floor is at about 1850 m depth, and a post-caldera lava dome was constructed on the southern caldera floor and partially merges with the southern caldera wall. Brothers volcano displays major submarine hydrothermal activity, including a large field of &quot;black smoker&quot; vents on the NW caldera wall and vents on the post-caldera dome.</obo:IAO_0000115>
        <oboInOwl:hasOBONamespace>GAZ</oboInOwl:hasOBONamespace>
        <oboInOwl:id>GAZ:00053836</oboInOwl:id>
        <rdfs:label>Brothers Volcano</rdfs:label>
    </owl:NamedIndividual>
    


    <!-- http://purl.obolibrary.org/obo/GAZ_00053837 -->

    <owl:NamedIndividual rdf:about="http://purl.obolibrary.org/obo/GAZ_00053837">
        <obo:RO_0001025 rdf:resource="http://purl.obolibrary.org/obo/GAZ_00007139"/>
        <obo:IAO_0000115>A submarine volcano that lies along the South Kermadec Ridge and consists of an elongated edifice with a 3 x 4 km wide caldera at the NE end whose rim reaches to 1150 m below sea level. A smaller caldera lies to the SW, and a satellitic cone, Cotton volcano, rises to 980 below sea level at the SW end of the 15 km-long complex. The flat-lying floor of the larger NE caldera lies 250-400 m below the caldera rim. Rhyodacitic pumice deposits mantle the caldera floor and walls, as well as the flanks of the volcano. Active hydrothermal venting has been observed on the lower part of the southern caldera wall.</obo:IAO_0000115>
        <oboInOwl:hasOBONamespace>GAZ</oboInOwl:hasOBONamespace>
        <oboInOwl:id>GAZ:00053837</oboInOwl:id>
        <rdfs:label>Healey Seamount</rdfs:label>
    </owl:NamedIndividual>
    


    <!-- http://purl.obolibrary.org/obo/GAZ_00053838 -->

    <owl:NamedIndividual rdf:about="http://purl.obolibrary.org/obo/GAZ_00053838">
        <obo:RO_0001025 rdf:resource="http://purl.obolibrary.org/obo/GAZ_00004765"/>
        <obo:IAO_0000115>A monogenetic volcanic field, which is a late Pleistocene to late Holocene in age, lies at the southern end of the Northland Peninsula and is overlain by New Zealand&apos;s largest city. More than 50 maars, tuff rings, small lava shields, and scoria cones have formed in the past 140,000 years in an elliptical volcanic field 29 km long in its largest (N-S) direction. The Auckland volcanic field has dominantly produced intraplate alkali basaltic to basantic rocks forming the northernmost of a group of Quaternary volcanic fields of the Auckland Intraplate Province.</obo:IAO_0000115>
        <oboInOwl:hasOBONamespace>GAZ</oboInOwl:hasOBONamespace>
        <oboInOwl:id>GAZ:00053838</oboInOwl:id>
        <rdfs:label>Auckland Volcanic Field</rdfs:label>
    </owl:NamedIndividual>
    


    <!-- http://purl.obolibrary.org/obo/GAZ_00053839 -->

    <owl:NamedIndividual rdf:about="http://purl.obolibrary.org/obo/GAZ_00053839">
        <obo:RO_0001025 rdf:resource="http://purl.obolibrary.org/obo/GAZ_00030233"/>
        <obo:IAO_0000115>A crater lake.</obo:IAO_0000115>
        <oboInOwl:hasOBONamespace>GAZ</oboInOwl:hasOBONamespace>
        <oboInOwl:id>GAZ:00053839</oboInOwl:id>
        <rdfs:label>Black Lake</rdfs:label>
    </owl:NamedIndividual>
    


    <!-- http://purl.obolibrary.org/obo/GAZ_00053840 -->

    <owl:NamedIndividual rdf:about="http://purl.obolibrary.org/obo/GAZ_00053840">
        <obo:RO_0001025 rdf:resource="http://purl.obolibrary.org/obo/GAZ_00030233"/>
        <obo:IAO_0000115>A crater lake.</obo:IAO_0000115>
        <oboInOwl:hasOBONamespace>GAZ</oboInOwl:hasOBONamespace>
        <oboInOwl:id>GAZ:00053840</oboInOwl:id>
        <rdfs:label>Green Lake</rdfs:label>
    </owl:NamedIndividual>
    


    <!-- http://purl.obolibrary.org/obo/GAZ_00053841 -->

    <owl:NamedIndividual rdf:about="http://purl.obolibrary.org/obo/GAZ_00053841">
        <obo:RO_0001025 rdf:resource="http://purl.obolibrary.org/obo/GAZ_00053842"/>
        <obo:IAO_0000115>An andesitic stratovolcano, is surrounded by a ring plain of debris-avalanche and lahar deposits that extend to the coast. The isolated Egmont volcanic center is located on the west coast of central North Island at the southern end of a volcanic arc extending NW along the Northland Peninsula. Egmont is the youngest and SE-most of a group of three volcanoes beginning with the Pleistocene Kaitoke Range. Fanthams Peak breaks the symmetry of Egmont on its south flank, and four lava domes are located on the lower north and south flanks.</obo:IAO_0000115>
        <oboInOwl:hasOBONamespace>GAZ</oboInOwl:hasOBONamespace>
        <oboInOwl:id>GAZ:00053841</oboInOwl:id>
        <rdfs:label>Mount Taranaki</rdfs:label>
    </owl:NamedIndividual>
    


    <!-- http://purl.obolibrary.org/obo/GAZ_00053842 -->

    <owl:NamedIndividual rdf:about="http://purl.obolibrary.org/obo/GAZ_00053842">
        <obo:RO_0001025 rdf:resource="http://purl.obolibrary.org/obo/GAZ_00008564"/>
        <obo:IAO_0000115>A national park located south of New Plymouth, close to the west coast of the North Island of New Zealand.</obo:IAO_0000115>
        <oboInOwl:hasOBONamespace>GAZ</oboInOwl:hasOBONamespace>
        <oboInOwl:id>GAZ:00053842</oboInOwl:id>
        <rdfs:label>Egmont National Park</rdfs:label>
    </owl:NamedIndividual>
    


    <!-- http://purl.obolibrary.org/obo/GAZ_00053843 -->

    <owl:NamedIndividual rdf:about="http://purl.obolibrary.org/obo/GAZ_00053843">
        <obo:RO_0001025 rdf:resource="http://purl.obolibrary.org/obo/GAZ_00053841"/>
        <obo:IAO_0000115>A secondary peak on Mount Taranaki.</obo:IAO_0000115>
        <oboInOwl:hasOBONamespace>GAZ</oboInOwl:hasOBONamespace>
        <oboInOwl:id>GAZ:00053843</oboInOwl:id>
        <rdfs:label>Fanthams Peak</rdfs:label>
    </owl:NamedIndividual>
    


    <!-- http://purl.obolibrary.org/obo/GAZ_00053844 -->

    <owl:NamedIndividual rdf:about="http://purl.obolibrary.org/obo/GAZ_00053844">
        <obo:RO_0001025 rdf:resource="http://purl.obolibrary.org/obo/GAZ_00004765"/>
        <obo:IAO_0000115>One of several mountain ranges in the North Island of New Zealand which form a ridge running parallel with the east coast of the island between East Cape and Wellington. The ridge is at its most pronounced in the southern part of the island, where it comprises the Rimutaka, Ruahine, and Tararua Ranges. The Tararuas run northeast-southwest for 80 km from near Palmerston North to the upper reaches of the Hutt Valley, where the northern tip of the Rimutaka Range begins. It is separated in the north from the southern end of the Ruahine Range by the Manawatu Gorge.</obo:IAO_0000115>
        <oboInOwl:hasOBONamespace>GAZ</oboInOwl:hasOBONamespace>
        <oboInOwl:id>GAZ:00053844</oboInOwl:id>
        <rdfs:label>Tararua Range</rdfs:label>
    </owl:NamedIndividual>
    


    <!-- http://purl.obolibrary.org/obo/GAZ_00053845 -->

    <owl:NamedIndividual rdf:about="http://purl.obolibrary.org/obo/GAZ_00053845">
        <obo:RO_0001025 rdf:resource="http://purl.obolibrary.org/obo/GAZ_00051945"/>
        <obo:IAO_0000115>A dominantly rhyolitic Volcanic Centre is surrounded by extensive ignimbrite and pyroclastic sheets produced during multiple caldera-forming eruptions. Numerous lava domes and craters erupted from two subparallel NE-SW-trending vent lineations form the Haroharo and Tarawera volcanic complexes. Lava domes of the Haroharo complex, at the northern end of the Okataina Volcanic Centre, occupy part of the 16 x 26 km Pleistocene Haroharo caldera, which formed incrementally between 300,000 and 50,000 years before present (BP). The oldest exposed rocks on the caldera floor are about 22,000 years old. The Tarawera complex at the southern end of Okataina consists of 11 rhyolitic lava domes and associated lava flows. The oldest domes were formed as late as about 15,000 years BP, and the youngest were formed in the Kaharoa eruption about 800 years BP. The NE-SW Tarawera vent lineation extends from the two dacitic cones of Maungaongaonga and Mangakakaramea on the SW to Mount Edgecumbe on the NE. Construction of the Haroharo and Tarawera complexes impounded lakes Rotoiti, Totoehu, Okataina, and Tarawera against the outer margins of the Okataina ring structure. A major hydrothermal area is located at Waimangu.</obo:IAO_0000115>
        <oboInOwl:hasOBONamespace>GAZ</oboInOwl:hasOBONamespace>
        <oboInOwl:id>GAZ:00053845</oboInOwl:id>
        <rdfs:label>Okataina Volcanic Centre</rdfs:label>
    </owl:NamedIndividual>
    


    <!-- http://purl.obolibrary.org/obo/GAZ_00053846 -->

    <owl:NamedIndividual rdf:about="http://purl.obolibrary.org/obo/GAZ_00053846">
        <rdf:type rdf:resource="http://purl.obolibrary.org/obo/ENVO_00000354"/>
        <obo:RO_0001025 rdf:resource="http://purl.obolibrary.org/obo/GAZ_00053845"/>
        <obo:IAO_0000115>A volcanic complex.</obo:IAO_0000115>
        <oboInOwl:hasOBONamespace>GAZ</oboInOwl:hasOBONamespace>
        <oboInOwl:id>GAZ:00053846</oboInOwl:id>
        <rdfs:label>Haroharo Volcanic Complex</rdfs:label>
    </owl:NamedIndividual>
    


    <!-- http://purl.obolibrary.org/obo/GAZ_00053847 -->

    <owl:NamedIndividual rdf:about="http://purl.obolibrary.org/obo/GAZ_00053847">
        <obo:RO_0001025 rdf:resource="http://purl.obolibrary.org/obo/GAZ_00053845"/>
        <obo:IAO_0000115>A volcanic mountain 24.1 km southeast of Rotorua in the North Island of New Zealand. It consists of a series of rhyolitic lava domes that were fissured down the middle by a basaltic eruption in 1886. The peaks are Ruawahia Peak, Tarawera Peak and Wahanga Peak. The summit is at 1111 m. The crater of the volcano is a series of chasms, running for 6 km northeast-southwest.</obo:IAO_0000115>
        <oboInOwl:hasOBONamespace>GAZ</oboInOwl:hasOBONamespace>
        <oboInOwl:id>GAZ:00053847</oboInOwl:id>
        <rdfs:label>Tarawera Volcanic Complex</rdfs:label>
    </owl:NamedIndividual>
    


    <!-- http://purl.obolibrary.org/obo/GAZ_00053848 -->

    <owl:NamedIndividual rdf:about="http://purl.obolibrary.org/obo/GAZ_00053848">
        <obo:RO_0001025 rdf:resource="http://purl.obolibrary.org/obo/GAZ_00051945"/>
        <obo:IAO_0000115>An extinct volcanic cone in the Bay of Plenty region of New Zealand 50 km east of Rotorua and three km east of Kawerau.</obo:IAO_0000115>
        <oboInOwl:hasOBONamespace>GAZ</oboInOwl:hasOBONamespace>
        <oboInOwl:id>GAZ:00053848</oboInOwl:id>
        <rdfs:label>Mount Edgecumbe</rdfs:label>
    </owl:NamedIndividual>
    


    <!-- http://purl.obolibrary.org/obo/GAZ_00053849 -->

    <owl:NamedIndividual rdf:about="http://purl.obolibrary.org/obo/GAZ_00053849">
        <obo:RO_0001025 rdf:resource="http://purl.obolibrary.org/obo/GAZ_00053845"/>
        <obo:IAO_0000115>A hydro thermal system created as the direct result of the volcanic eruption of Mount Tarawera on 1886-06-10. It includes Lake Rotomahana, the former site of the Pink and White Terraces.</obo:IAO_0000115>
        <oboInOwl:hasOBONamespace>GAZ</oboInOwl:hasOBONamespace>
        <oboInOwl:id>GAZ:00053849</oboInOwl:id>
        <rdfs:label>Waimangu Volcanic Rift Valley</rdfs:label>
    </owl:NamedIndividual>
    


    <!-- http://purl.obolibrary.org/obo/GAZ_00053851 -->

    <owl:NamedIndividual rdf:about="http://purl.obolibrary.org/obo/GAZ_00053851">
        <obo:RO_0001025 rdf:resource="http://purl.obolibrary.org/obo/GAZ_00051945"/>
        <obo:IAO_0000115>An active geothermal area just north of the Reporoa caldera in New Zealand&apos;s Taupo Volcanic Zone. The area has many hot springs noted for their colourful appearance, in addition to the Lady Knox Geyser.</obo:IAO_0000115>
        <oboInOwl:hasOBONamespace>GAZ</oboInOwl:hasOBONamespace>
        <oboInOwl:id>GAZ:00053851</oboInOwl:id>
        <rdfs:label>Wai-O-Tapu</rdfs:label>
    </owl:NamedIndividual>
    


    <!-- http://purl.obolibrary.org/obo/GAZ_00053852 -->

    <owl:NamedIndividual rdf:about="http://purl.obolibrary.org/obo/GAZ_00053852">
        <obo:RO_0001025 rdf:resource="http://purl.obolibrary.org/obo/GAZ_00053851"/>
        <obo:IAO_0000115>A geyser in the Wai-o-Tapu area of the Taupo Volcanic Zone in New Zealand.</obo:IAO_0000115>
        <oboInOwl:hasOBONamespace>GAZ</oboInOwl:hasOBONamespace>
        <oboInOwl:id>GAZ:00053852</oboInOwl:id>
        <rdfs:label>Lady Knox Geyser</rdfs:label>
    </owl:NamedIndividual>
    


    <!-- http://purl.obolibrary.org/obo/GAZ_00053853 -->

    <owl:NamedIndividual rdf:about="http://purl.obolibrary.org/obo/GAZ_00053853">
        <obo:RO_0001025 rdf:resource="http://purl.obolibrary.org/obo/GAZ_00053851"/>
        <obo:IAO_0000115>A small lake in the Wai-O-Tapu geothermal area in the Waikato region of the North Island of New Zealand. The lake is formed by the surfacing of one of the largest hot springs in the area. It is roughly circular with a diameter of 65m and a depth of 62m. The surface temperature of the water is 74degC and bubbles of carbon dioxide can be seen continuously rising to the surface, giving the pool its name.</obo:IAO_0000115>
        <oboInOwl:hasOBONamespace>GAZ</oboInOwl:hasOBONamespace>
        <oboInOwl:id>GAZ:00053853</oboInOwl:id>
        <rdfs:label>Champagne Pool</rdfs:label>
    </owl:NamedIndividual>
    


    <!-- http://purl.obolibrary.org/obo/GAZ_00053854 -->

    <owl:NamedIndividual rdf:about="http://purl.obolibrary.org/obo/GAZ_00053854">
        <obo:RO_0001025 rdf:resource="http://purl.obolibrary.org/obo/GAZ_00051945"/>
        <obo:IAO_0000115>A highly active geothermal area most notable for its series of fault-stepped sinter terraces, located in a valley north of Taupo on the banks of the Waikato River in the Taupo Volcanic Zone, New Zealand.</obo:IAO_0000115>
        <oboInOwl:hasOBONamespace>GAZ</oboInOwl:hasOBONamespace>
        <oboInOwl:id>GAZ:00053854</oboInOwl:id>
        <rdfs:label>Orakei Korako</rdfs:label>
    </owl:NamedIndividual>
    


    <!-- http://purl.obolibrary.org/obo/GAZ_00053855 -->

    <owl:NamedIndividual rdf:about="http://purl.obolibrary.org/obo/GAZ_00053855">
        <obo:RO_0001025 rdf:resource="http://purl.obolibrary.org/obo/GAZ_00051945"/>
        <obo:IAO_0000115>A geothermal area a few km north of Taupo, in the centre of the North Island of New Zealand, on the Waikato River.</obo:IAO_0000115>
        <oboInOwl:hasOBONamespace>GAZ</oboInOwl:hasOBONamespace>
        <oboInOwl:id>GAZ:00053855</oboInOwl:id>
        <rdfs:label>Wairakei Geothermal Field</rdfs:label>
    </owl:NamedIndividual>
    


    <!-- http://purl.obolibrary.org/obo/GAZ_00053856 -->

    <owl:NamedIndividual rdf:about="http://purl.obolibrary.org/obo/GAZ_00053856">
        <obo:RO_0001025 rdf:resource="http://purl.obolibrary.org/obo/GAZ_00051945"/>
        <obo:IAO_0000115>A small but highly active geothermal field covering about 50,000 m?, close to State Highway 1 a few km north of Taupo, New Zealand.</obo:IAO_0000115>
        <oboInOwl:hasOBONamespace>GAZ</oboInOwl:hasOBONamespace>
        <oboInOwl:id>GAZ:00053856</oboInOwl:id>
        <rdfs:label>Craters of the Moon Geothermal Field</rdfs:label>
    </owl:NamedIndividual>
    


    <!-- http://purl.obolibrary.org/obo/GAZ_00053857 -->

    <owl:NamedIndividual rdf:about="http://purl.obolibrary.org/obo/GAZ_00053857">
        <obo:RO_0001025 rdf:resource="http://purl.obolibrary.org/obo/GAZ_00051945"/>
        <obo:IAO_0000115>A dormant stratovolcano, reaching 1,088 m above sea level, situated within the Taupo caldera towards the southern end of the Taupo Volcanic Zone. It is 6 km E of the town of Taupo, New Zealand, next to the northeastern shore of Lake Taupo.</obo:IAO_0000115>
        <oboInOwl:hasOBONamespace>GAZ</oboInOwl:hasOBONamespace>
        <oboInOwl:id>GAZ:00053857</oboInOwl:id>
        <rdfs:label>Mount Tauhara</rdfs:label>
    </owl:NamedIndividual>
    


    <!-- http://purl.obolibrary.org/obo/GAZ_00053858 -->

    <owl:NamedIndividual rdf:about="http://purl.obolibrary.org/obo/GAZ_00053858">
        <obo:RO_0001025 rdf:resource="http://purl.obolibrary.org/obo/GAZ_00007545"/>
        <obo:IAO_0000115>A stratovolcanic complex in the North Island of New Zealand. It is located 20 km to the southwest of Lake Taupo, and is the northernmost of the three active volcanoes that dominate the landscape of the central North Island. A large andesitic volcanic massif, located immediately NE of Ruapehu volcano, that is composed of more than a dozen composite cones constructed over a period of 275,000 years. Vents along a NE-trending zone extending from Saddle Cone (below Ruapehu volcano) to Te Mari crater (including vents at the present-day location of Ngauruhoe) were active during a several hundred year long period around 10,000 years ago, producing the largest known eruptions at the Tongariro complex during the Holocene. North Crater stratovolcano, one of the largest features of the massif, is truncated by a broad, shallow crater filled by a solidified lava lake that is cut on the NW side by a small explosion crater. The youngest cone of the complex, Ngauruhoe, has grown to become the highest peak of the massif since its birth about 2500 years ago.</obo:IAO_0000115>
        <oboInOwl:hasOBONamespace>GAZ</oboInOwl:hasOBONamespace>
        <oboInOwl:id>GAZ:00053858</oboInOwl:id>
        <rdfs:label>Mount Tongariro</rdfs:label>
    </owl:NamedIndividual>
    


    <!-- http://purl.obolibrary.org/obo/GAZ_00053859 -->

    <owl:NamedIndividual rdf:about="http://purl.obolibrary.org/obo/GAZ_00053859">
        <obo:RO_0001025 rdf:resource="http://purl.obolibrary.org/obo/GAZ_00053858"/>
        <obo:IAO_0000115>A crater lake.</obo:IAO_0000115>
        <oboInOwl:hasOBONamespace>GAZ</oboInOwl:hasOBONamespace>
        <oboInOwl:id>GAZ:00053859</oboInOwl:id>
        <rdfs:label>Blue Lake</rdfs:label>
    </owl:NamedIndividual>
    


    <!-- http://purl.obolibrary.org/obo/GAZ_00053860 -->

    <owl:NamedIndividual rdf:about="http://purl.obolibrary.org/obo/GAZ_00053860">
        <obo:RO_0001025 rdf:resource="http://purl.obolibrary.org/obo/GAZ_00053858"/>
        <obo:IAO_0000115>A crater.</obo:IAO_0000115>
        <oboInOwl:hasOBONamespace>GAZ</oboInOwl:hasOBONamespace>
        <oboInOwl:id>GAZ:00053860</oboInOwl:id>
        <rdfs:label>Red Crater</rdfs:label>
    </owl:NamedIndividual>
    


    <!-- http://purl.obolibrary.org/obo/GAZ_00053861 -->

    <owl:NamedIndividual rdf:about="http://purl.obolibrary.org/obo/GAZ_00053861">
        <obo:RO_0001025 rdf:resource="http://purl.obolibrary.org/obo/GAZ_00053858"/>
        <obo:IAO_0000115>Crater lakes.</obo:IAO_0000115>
        <oboInOwl:hasOBONamespace>GAZ</oboInOwl:hasOBONamespace>
        <oboInOwl:id>GAZ:00053861</oboInOwl:id>
        <rdfs:label>Emerald Lakes</rdfs:label>
    </owl:NamedIndividual>
    


    <!-- http://purl.obolibrary.org/obo/GAZ_00053862 -->

    <owl:NamedIndividual rdf:about="http://purl.obolibrary.org/obo/GAZ_00053862">
        <obo:RO_0001025 rdf:resource="http://purl.obolibrary.org/obo/GAZ_00051945"/>
        <obo:IAO_0000115>A caldera occupying the Reporoa-Broadlands basin, lies near the western margin of the Taupo volcanic zone SSW of the Okataina volcanic center. Reporoa caldera formed about 230,000 years ago during the eruption of the voluminous ca. 100 cu km Kaingaroa Ignimbrite. Large slump scallops cut the northern caldera rim; on the south the rim is buried by sediments. The Deer Hill rhyolitic lava dome was erupted after caldera collapse on the southern rim; two other rhyolitic domes, Kairuru and Pukekahu, were emplaced within the caldera along a possible ring fault. The active Reporoa hydrothermal field lies within the caldera, and the Waiotapu and Broadlands (Ohaki) hydrothermal fields lie occur north and south of the poorly defined caldera margin.</obo:IAO_0000115>
        <oboInOwl:hasOBONamespace>GAZ</oboInOwl:hasOBONamespace>
        <oboInOwl:id>GAZ:00053862</oboInOwl:id>
        <rdfs:label>Reporoa Caldera</rdfs:label>
    </owl:NamedIndividual>
    


    <!-- http://purl.obolibrary.org/obo/GAZ_00053863 -->

    <owl:NamedIndividual rdf:about="http://purl.obolibrary.org/obo/GAZ_00053863">
        <obo:RO_0001025 rdf:resource="http://purl.obolibrary.org/obo/GAZ_00051945"/>
        <obo:IAO_0000115>A caldera that partially overlaps with the Taupo caldera on the south and was formed during the eruption of the Whakamaru Group ignimbrites between about 340 and 330 ka.</obo:IAO_0000115>
        <oboInOwl:hasOBONamespace>GAZ</oboInOwl:hasOBONamespace>
        <oboInOwl:id>GAZ:00053863</oboInOwl:id>
        <rdfs:label>Whakamaru Caldera</rdfs:label>
    </owl:NamedIndividual>
    


    <!-- http://purl.obolibrary.org/obo/GAZ_00053864 -->

    <owl:NamedIndividual rdf:about="http://purl.obolibrary.org/obo/GAZ_00053864">
        <obo:RO_0001025 rdf:resource="http://purl.obolibrary.org/obo/GAZ_00051945"/>
        <obo:IAO_0000115>A caldera formed sometime after 230 thousand years ago (ka) in the NE corner of the 30 x 40 km Whakamaru caldera, which is the largest of the Taupo volcanic zone.</obo:IAO_0000115>
        <oboInOwl:hasOBONamespace>GAZ</oboInOwl:hasOBONamespace>
        <oboInOwl:id>GAZ:00053864</oboInOwl:id>
        <rdfs:label>Maroa Caldara</rdfs:label>
    </owl:NamedIndividual>
    


    <!-- http://purl.obolibrary.org/obo/GAZ_00053865 -->

    <owl:NamedIndividual rdf:about="http://purl.obolibrary.org/obo/GAZ_00053865">
        <obo:RO_0001025 rdf:resource="http://purl.obolibrary.org/obo/GAZ_00007139"/>
        <obo:IAO_0000115>A submarine volcano lies near the southern end of the Southern Kermadec arc. This basaltic and dacitic stratovolcano consists of a basal substrate of massive lava flows, pillow lavas, and pillow tubes overlain by volcaniclastic sediments. Craters occupy the complex crest of the volcano. Clark is the southernmost volcano of the submarine chain that displays hydrothermal activity.</obo:IAO_0000115>
        <oboInOwl:hasOBONamespace>GAZ</oboInOwl:hasOBONamespace>
        <oboInOwl:id>GAZ:00053865</oboInOwl:id>
        <rdfs:label>Clark Seamount</rdfs:label>
    </owl:NamedIndividual>
    


    <!-- http://purl.obolibrary.org/obo/GAZ_00053866 -->

    <owl:NamedIndividual rdf:about="http://purl.obolibrary.org/obo/GAZ_00053866">
        <obo:RO_0001025 rdf:resource="http://purl.obolibrary.org/obo/GAZ_00007139"/>
        <obo:IAO_0000115>A submarine volcano in the southern Kermadec arc rises to within 600 m of the sea surface. Tangaroa lies between Clark and Rumble V submarine volcanoes near the southern end of the Kermadec arc and is one of more than a half dozen volcanoes in this part of the arc showing evidence for active hydrothermal vent fields.</obo:IAO_0000115>
        <oboInOwl:hasOBONamespace>GAZ</oboInOwl:hasOBONamespace>
        <oboInOwl:id>GAZ:00053866</oboInOwl:id>
        <rdfs:label>Tangaroa Seamount</rdfs:label>
    </owl:NamedIndividual>
    


    <!-- http://purl.obolibrary.org/obo/GAZ_00053867 -->

    <owl:NamedIndividual rdf:about="http://purl.obolibrary.org/obo/GAZ_00053867">
        <obo:RO_0001025 rdf:resource="http://purl.obolibrary.org/obo/GAZ_00007139"/>
        <obo:IAO_0000115>A submarine volcano was discovered in 1992 at the southern end of the South Kermadec Ridge. It is the southernmost of a group of seamounts on the southern Kermadec Ridge, known as the Rumbles, rises more than 2000 m to nearly 400 m below the sea surface and shows a pristine morphology. Andesitic and basaltic-andesite rocks have been dredged from Rumble V, which lies 17 km ESE of Rumble IV. A large plume of gas bubbles was acoustically detected rising from the summit of Rumble V in 1992, and subsequent expeditions detected evidence of vigorous hydrothermal activity.</obo:IAO_0000115>
        <oboInOwl:hasOBONamespace>GAZ</oboInOwl:hasOBONamespace>
        <oboInOwl:id>GAZ:00053867</oboInOwl:id>
        <rdfs:label>Rumble V</rdfs:label>
    </owl:NamedIndividual>
    


    <!-- http://purl.obolibrary.org/obo/GAZ_00053868 -->

    <owl:NamedIndividual rdf:about="http://purl.obolibrary.org/obo/GAZ_00053868">
        <obo:RO_0001025 rdf:resource="http://purl.obolibrary.org/obo/GAZ_00007139"/>
        <obo:IAO_0000115>The largest of the Rumbles seamount group along the South Kermadec Ridge, rises 2300 m from the sea floor to within about 200 m of the sea surface. Fresh-looking andesitic rocks have been dredged from its summit and basaltic lava from its flanks. Rumble III has been the source of several submarine eruptions detected by hydrophone signals. Early surveys placed its depth at 117 m, and later depths of about 200 m, 140 m, and 220 m were determined.</obo:IAO_0000115>
        <oboInOwl:hasOBONamespace>GAZ</oboInOwl:hasOBONamespace>
        <oboInOwl:id>GAZ:00053868</oboInOwl:id>
        <rdfs:label>Rumble III</rdfs:label>
    </owl:NamedIndividual>
    


    <!-- http://purl.obolibrary.org/obo/GAZ_00053869 -->

    <owl:NamedIndividual rdf:about="http://purl.obolibrary.org/obo/GAZ_00053869">
        <obo:RO_0001025 rdf:resource="http://purl.obolibrary.org/obo/GAZ_00007139"/>
        <obo:IAO_0000115>A seamount (submarine volcano) located NW of Rumble II East, displays evidence of hydrothermal activity. Rumble II West contains a 2.5-3 km wide summit caldera about 200 m deep with a central cone and is about twice the volume of Rumble II East. Rumble II West rises 1800 m from the sea floor to within 1200 m of the sea surface and is the deepest of the Rumble group seamounts. Satellitic cones are found on the flanks of the volcano. Recent lava flows originating from near the caldera rim with little or no sediment cover blanket the western flanks.</obo:IAO_0000115>
        <oboInOwl:hasOBONamespace>GAZ</oboInOwl:hasOBONamespace>
        <oboInOwl:id>GAZ:00053869</oboInOwl:id>
        <rdfs:label>Rumble II West</rdfs:label>
    </owl:NamedIndividual>
    


    <!-- http://purl.obolibrary.org/obo/GAZ_00053870 -->

    <owl:NamedIndividual rdf:about="http://purl.obolibrary.org/obo/GAZ_00053870">
        <obo:RO_0001025 rdf:resource="http://purl.obolibrary.org/obo/GAZ_00030230"/>
        <obo:IAO_0000115>A white anhydrite cone some 6-8 m high, formed at 167 m depth by discharge of thermal waters at the ocean floor. It was discovered in 1987-02 using the diving vessel Soucoup carried on the RV Calypso (Sarano and others, 1989). It lies within one of the &apos;bubble zones&apos; extending in a line from White Island to Whale Island in the Bay of Plenty.</obo:IAO_0000115>
        <oboInOwl:hasOBONamespace>GAZ</oboInOwl:hasOBONamespace>
        <oboInOwl:id>GAZ:00053870</oboInOwl:id>
        <rdfs:label>Calypso Mound</rdfs:label>
    </owl:NamedIndividual>
    


    <!-- http://purl.obolibrary.org/obo/GAZ_00053871 -->

    <owl:NamedIndividual rdf:about="http://purl.obolibrary.org/obo/GAZ_00053871">
        <obo:RO_0001025 rdf:resource="http://purl.obolibrary.org/obo/GAZ_00007545"/>
        <obo:IAO_0000115>A volcanic peak in the North Island Volcanic Plateau, located to the north of Mount Tongariro, between Tongariro and Lake Taupo. Lake Rotoaira lies immediately to the west of Pihanga, and the smaller Lake Rotopounamu is at the north-west foot of the mountain. Mt. Pihanga and Lake Rotopounamu are part of the 5,129ha Pihanga Scenic Reserve, which in 1975 was added to the Tongariro National Park.</obo:IAO_0000115>
        <oboInOwl:hasOBONamespace>GAZ</oboInOwl:hasOBONamespace>
        <oboInOwl:id>GAZ:00053871</oboInOwl:id>
        <rdfs:label>Mount Pihanga</rdfs:label>
    </owl:NamedIndividual>
    


    <!-- http://purl.obolibrary.org/obo/GAZ_00053872 -->

    <owl:NamedIndividual rdf:about="http://purl.obolibrary.org/obo/GAZ_00053872">
        <obo:RO_0001025 rdf:resource="http://purl.obolibrary.org/obo/GAZ_00007545"/>
        <obo:IAO_0000115>Two crater lakes in New Zealand&apos;s Tongariro National Park. They fill two of a series of explosion craters on the Tama Saddle between Mount Ruapehu and Mount Ngaruahoe.</obo:IAO_0000115>
        <oboInOwl:hasOBONamespace>GAZ</oboInOwl:hasOBONamespace>
        <oboInOwl:id>GAZ:00053872</oboInOwl:id>
        <rdfs:label>Tama Lakes</rdfs:label>
    </owl:NamedIndividual>
    


    <!-- http://purl.obolibrary.org/obo/GAZ_00053873 -->

    <owl:NamedIndividual rdf:about="http://purl.obolibrary.org/obo/GAZ_00053873">
        <rdf:type rdf:resource="http://purl.obolibrary.org/obo/ENVO_00000106"/>
        <obo:RO_0001025 rdf:resource="http://purl.obolibrary.org/obo/GAZ_00004765"/>
        <obo:IAO_0000115>A range of hills to the south of Auckland in New Zealand&apos;s North Island. They are located 40 km southeast of Auckland, close to the town of Pukekohe. State Highway 1 here reaches its highest point between Auckland and Tirau in the eastern Waikato Region, 134 km to the southeast.</obo:IAO_0000115>
        <oboInOwl:hasOBONamespace>GAZ</oboInOwl:hasOBONamespace>
        <oboInOwl:id>GAZ:00053873</oboInOwl:id>
        <rdfs:label>Bombay Hills</rdfs:label>
    </owl:NamedIndividual>
    


    <!-- http://purl.obolibrary.org/obo/GAZ_00053874 -->

    <owl:NamedIndividual rdf:about="http://purl.obolibrary.org/obo/GAZ_00053874">
        <obo:RO_0001025 rdf:resource="http://purl.obolibrary.org/obo/GAZ_00004781"/>
        <obo:IAO_0000115>An extinct volcano located in the Waikato region of New Zealand&apos;s North Island. It rises to 962 m and is the highest peak in the Waikato region. It is 22 km to the west of Te Awamutu and eight km from the small settlement of Pirongia, and lies in a forest park. It is clearly visible from the Tasman Sea, being just 25 km from the coast at Aotea Harbour.</obo:IAO_0000115>
        <oboInOwl:hasOBONamespace>GAZ</oboInOwl:hasOBONamespace>
        <oboInOwl:id>GAZ:00053874</oboInOwl:id>
        <rdfs:label>Mount Pirongia</rdfs:label>
    </owl:NamedIndividual>
    


    <!-- http://purl.obolibrary.org/obo/GAZ_00055569 -->

    <owl:NamedIndividual rdf:about="http://purl.obolibrary.org/obo/GAZ_00055569">
        <obo:RO_0001025 rdf:resource="http://purl.obolibrary.org/obo/GAZ_00007139"/>
        <obo:IAO_0000115>A seamount.</obo:IAO_0000115>
        <oboInOwl:hasOBONamespace>GAZ</oboInOwl:hasOBONamespace>
        <oboInOwl:id>GAZ:00055569</oboInOwl:id>
        <rdfs:label>Rumble I</rdfs:label>
    </owl:NamedIndividual>
    


    <!-- http://purl.obolibrary.org/obo/GAZ_00055570 -->

    <owl:NamedIndividual rdf:about="http://purl.obolibrary.org/obo/GAZ_00055570">
        <obo:RO_0001025 rdf:resource="http://purl.obolibrary.org/obo/GAZ_00007139"/>
        <obo:IAO_0000115>A seamount.</obo:IAO_0000115>
        <oboInOwl:hasOBONamespace>GAZ</oboInOwl:hasOBONamespace>
        <oboInOwl:id>GAZ:00055570</oboInOwl:id>
        <rdfs:label>Rumble IV</rdfs:label>
    </owl:NamedIndividual>
    


    <!-- http://purl.obolibrary.org/obo/GAZ_00055985 -->

    <owl:NamedIndividual rdf:about="http://purl.obolibrary.org/obo/GAZ_00055985">
        <obo:RO_0001025 rdf:resource="http://purl.obolibrary.org/obo/GAZ_00044917"/>
        <obo:IAO_0000115>A pyroclastic cone.</obo:IAO_0000115>
        <oboInOwl:hasOBONamespace>GAZ</oboInOwl:hasOBONamespace>
        <oboInOwl:id>GAZ:00055985</oboInOwl:id>
        <rdfs:label>Mount Galloway</rdfs:label>
    </owl:NamedIndividual>
    


    <!-- http://purl.obolibrary.org/obo/GAZ_00055994 -->

    <owl:NamedIndividual rdf:about="http://purl.obolibrary.org/obo/GAZ_00055994">
        <obo:RO_0001025 rdf:resource="http://purl.obolibrary.org/obo/GAZ_00044917"/>
        <obo:IAO_0000115>A pyroclastic cone.</obo:IAO_0000115>
        <oboInOwl:hasOBONamespace>GAZ</oboInOwl:hasOBONamespace>
        <oboInOwl:id>GAZ:00055994</oboInOwl:id>
        <rdfs:label>Mount Waterhouse</rdfs:label>
    </owl:NamedIndividual>
    


    <!-- http://purl.obolibrary.org/obo/GAZ_00056646 -->

    <owl:NamedIndividual rdf:about="http://purl.obolibrary.org/obo/GAZ_00056646">
        <obo:RO_0001025 rdf:resource="http://purl.obolibrary.org/obo/GAZ_00030217"/>
        <obo:IAO_0000115>A national park located in the South Island of New Zealand near the town of Twizel. Aoraki/Mount Cook village lies within the park.</obo:IAO_0000115>
        <oboInOwl:hasOBONamespace>GAZ</oboInOwl:hasOBONamespace>
        <oboInOwl:id>GAZ:00056646</oboInOwl:id>
        <rdfs:label>Mount Cook National Park</rdfs:label>
    </owl:NamedIndividual>
    


    <!-- http://purl.obolibrary.org/obo/GAZ_00056647 -->

    <owl:NamedIndividual rdf:about="http://purl.obolibrary.org/obo/GAZ_00056647">
        <obo:RO_0001025 rdf:resource="http://purl.obolibrary.org/obo/GAZ_00030217"/>
        <obo:IAO_0000115>A national park located in New Zealand&apos;s South Island.</obo:IAO_0000115>
        <oboInOwl:hasOBONamespace>GAZ</oboInOwl:hasOBONamespace>
        <oboInOwl:id>GAZ:00056647</oboInOwl:id>
        <rdfs:label>Westland Tai Poutini National Park</rdfs:label>
    </owl:NamedIndividual>
    


    <!-- http://purl.obolibrary.org/obo/GAZ_00056648 -->

    <owl:NamedIndividual rdf:about="http://purl.obolibrary.org/obo/GAZ_00056648">
        <obo:RO_0001025 rdf:resource="http://purl.obolibrary.org/obo/GAZ_00030217"/>
        <obo:IAO_0000115>A national park located in the South Island of New Zealand.</obo:IAO_0000115>
        <oboInOwl:hasOBONamespace>GAZ</oboInOwl:hasOBONamespace>
        <oboInOwl:id>GAZ:00056648</oboInOwl:id>
        <rdfs:label>Mount Aspiring National Park</rdfs:label>
    </owl:NamedIndividual>
    


    <!-- http://purl.obolibrary.org/obo/GAZ_00056649 -->

    <owl:NamedIndividual rdf:about="http://purl.obolibrary.org/obo/GAZ_00056649">
        <obo:RO_0001025 rdf:resource="http://purl.obolibrary.org/obo/GAZ_00056646"/>
        <obo:IAO_0000115>The largest of several glaciers which flow south and east towards the Mackenzie Basin from the Southern Alps in New Zealand&apos;s South Island. It is 29 km long and as much as 4 km wide, and is entirely within the borders of Aoraki/Mount Cook National Park. The depth at its most is 600 meters. The Tasman flows south from the southern slopes of the Minarets peak, along the eastern flank of Aoraki/Mount Cook, the peak of which is only five km from the glacier. It is almost met partway along its length by the meltwater of the Murchison Glacier, which approaches from the northeast before turning to flow beside the Tasman Glacier outside the moraine wall. The waters from both these glaciers pool at the end of the glacier in Lake Tasman, before flowing south to join the outflow from the nearby Hooker and Mueller Glaciers in the wide valley of the Tasman River, whose braided streams flow south into Lake Pukaki. They eventually flow into the Waitaki River and to the Pacific Ocean north of Oamaru.</obo:IAO_0000115>
        <oboInOwl:hasOBONamespace>GAZ</oboInOwl:hasOBONamespace>
        <oboInOwl:id>GAZ:00056649</oboInOwl:id>
        <rdfs:label>Tasman Glacier</rdfs:label>
    </owl:NamedIndividual>
    


    <!-- http://purl.obolibrary.org/obo/GAZ_00056650 -->

    <owl:NamedIndividual rdf:about="http://purl.obolibrary.org/obo/GAZ_00056650">
        <obo:RO_0001025 rdf:resource="http://purl.obolibrary.org/obo/GAZ_00056646"/>
        <obo:IAO_0000115>An 18 km long glacier flowing through Aoraki/Mount Cook National Park in the South Island of New Zealand. Lying to the east of Aoraki/Mount Cook, high in the Southern Alps, it flows southwestwards. The Murchison River, which takes its meltwater, flows under the larger Tasman Glacier to the south.</obo:IAO_0000115>
        <oboInOwl:hasOBONamespace>GAZ</oboInOwl:hasOBONamespace>
        <oboInOwl:id>GAZ:00056650</oboInOwl:id>
        <rdfs:label>Murchison Glacier</rdfs:label>
    </owl:NamedIndividual>
    


    <!-- http://purl.obolibrary.org/obo/GAZ_00056651 -->

    <owl:NamedIndividual rdf:about="http://purl.obolibrary.org/obo/GAZ_00056651">
        <obo:RO_0001025 rdf:resource="http://purl.obolibrary.org/obo/GAZ_00056646"/>
        <obo:IAO_0000115>A glacial lake.</obo:IAO_0000115>
        <oboInOwl:hasOBONamespace>GAZ</oboInOwl:hasOBONamespace>
        <oboInOwl:id>GAZ:00056651</oboInOwl:id>
        <rdfs:label>Tasman Lake</rdfs:label>
    </owl:NamedIndividual>
    


    <!-- http://purl.obolibrary.org/obo/GAZ_00056652 -->

    <owl:NamedIndividual rdf:about="http://purl.obolibrary.org/obo/GAZ_00056652">
        <obo:RO_0001025 rdf:resource="http://purl.obolibrary.org/obo/GAZ_00056646"/>
        <obo:IAO_0000115>One of several glaciers close to the slopes of Aoraki/Mount Cook in the Southern Alps of New Zealand. Though not as large as its neighbour, the Tasman Glacier, it is still impressive, and is some 11 km in length. It is on the southwestern slopes of Aoraki/Mt Cook, and is the source of the Hooker River, a small tributary of the Tasman River, which flows into Lake Pukaki.</obo:IAO_0000115>
        <oboInOwl:hasOBONamespace>GAZ</oboInOwl:hasOBONamespace>
        <oboInOwl:id>GAZ:00056652</oboInOwl:id>
        <rdfs:label>Hooker Glacier</rdfs:label>
    </owl:NamedIndividual>
    


    <!-- http://purl.obolibrary.org/obo/GAZ_00056653 -->

    <owl:NamedIndividual rdf:about="http://purl.obolibrary.org/obo/GAZ_00056653">
        <obo:RO_0001025 rdf:resource="http://purl.obolibrary.org/obo/GAZ_00056646"/>
        <obo:IAO_0000115>A 13 km long glacier flowing through Aoraki/Mount Cook National Park in the South Island of New Zealand. It lies to the south of Aoraki/Mount Cook, high in the Southern Alps, and flows north. Its meltwaters eventually join the Tasman River.</obo:IAO_0000115>
        <oboInOwl:hasOBONamespace>GAZ</oboInOwl:hasOBONamespace>
        <oboInOwl:id>GAZ:00056653</oboInOwl:id>
        <rdfs:label>Mueller Glacier</rdfs:label>
    </owl:NamedIndividual>
    


    <!-- http://purl.obolibrary.org/obo/GAZ_00057526 -->

    <owl:NamedIndividual rdf:about="http://purl.obolibrary.org/obo/GAZ_00057526">
        <obo:RO_0001025 rdf:resource="http://purl.obolibrary.org/obo/GAZ_00047054"/>
        <obo:IAO_0000115>A lake located in the Mackenzie Basin of New Zealand&apos;s South Island, between the much larger lakes Tekapo and Pukaki, to the north of Lake Tekapo township.</obo:IAO_0000115>
        <oboInOwl:hasOBONamespace>GAZ</oboInOwl:hasOBONamespace>
        <oboInOwl:id>GAZ:00057526</oboInOwl:id>
        <rdfs:label>Lake Alexandrina</rdfs:label>
    </owl:NamedIndividual>
    


    <!-- http://purl.obolibrary.org/obo/GAZ_00057726 -->

    <owl:NamedIndividual rdf:about="http://purl.obolibrary.org/obo/GAZ_00057726">
        <obo:RO_0001025 rdf:resource="http://purl.obolibrary.org/obo/GAZ_00029953"/>
        <obo:IAO_0000115>A barren desert-like environment in New Zealand, located in the Ruapehu District on the North Island Volcanic Plateau; to the east of the three active peaks of Mount Tongariro, Mount Ngauruhoe, and Mount Ruapehu, and to the west of the Kaimanawa Range.</obo:IAO_0000115>
        <oboInOwl:hasOBONamespace>GAZ</oboInOwl:hasOBONamespace>
        <oboInOwl:id>GAZ:00057726</oboInOwl:id>
        <rdfs:label>Rangipo Desert</rdfs:label>
    </owl:NamedIndividual>
    


    <!-- http://purl.obolibrary.org/obo/GAZ_00057727 -->

    <owl:NamedIndividual rdf:about="http://purl.obolibrary.org/obo/GAZ_00057727">
        <obo:RO_0001025 rdf:resource="http://purl.obolibrary.org/obo/GAZ_00004765"/>
        <obo:IAO_0000115>A mountain range located in the central North Island of New Zealand. They extend for 50 km in a northeast/southwest direction through largely uninhabited country to the south of Lake Taupo, east of the &quot;Desert Road&quot;. Their slopes form part of the North Island Volcanic Plateau.</obo:IAO_0000115>
        <oboInOwl:hasOBONamespace>GAZ</oboInOwl:hasOBONamespace>
        <oboInOwl:id>GAZ:00057727</oboInOwl:id>
        <rdfs:label>Kaimanawa Range</rdfs:label>
    </owl:NamedIndividual>
    


    <!-- http://purl.obolibrary.org/obo/GAZ_00058645 -->

    <owl:NamedIndividual rdf:about="http://purl.obolibrary.org/obo/GAZ_00058645">
        <obo:RO_0001025 rdf:resource="http://purl.obolibrary.org/obo/GAZ_00004777"/>
        <obo:IAO_0000115>A lake in the Westland region of the South Island of New Zealand. It is located in the Southern Alps and is fed by a mountain stream. Another stream links the lake with the Perth River.</obo:IAO_0000115>
        <oboInOwl:hasOBONamespace>GAZ</oboInOwl:hasOBONamespace>
        <oboInOwl:id>GAZ:00058645</oboInOwl:id>
        <rdfs:label>Abel Lake</rdfs:label>
    </owl:NamedIndividual>
    


    <!-- http://purl.obolibrary.org/obo/GAZ_00058646 -->

    <owl:NamedIndividual rdf:about="http://purl.obolibrary.org/obo/GAZ_00058646">
        <obo:RO_0001025 rdf:resource="http://purl.obolibrary.org/obo/GAZ_00004764"/>
        <obo:IAO_0000115>A system of limestone (karst) caves on the western shore of Lake Te Anau, in the southwest of New Zealand.</obo:IAO_0000115>
        <oboInOwl:hasOBONamespace>GAZ</oboInOwl:hasOBONamespace>
        <oboInOwl:id>GAZ:00058646</oboInOwl:id>
        <rdfs:label>Te Ana-au Caves</rdfs:label>
    </owl:NamedIndividual>
    


    <!-- http://purl.obolibrary.org/obo/GAZ_00058647 -->

    <owl:NamedIndividual rdf:about="http://purl.obolibrary.org/obo/GAZ_00058647">
        <rdf:type rdf:resource="http://purl.obolibrary.org/obo/ENVO_00000475"/>
        <obo:RO_0001025 rdf:resource="http://purl.obolibrary.org/obo/GAZ_00047041"/>
        <obo:IAO_0000115>An arm of Lake Manapouri.</obo:IAO_0000115>
        <oboInOwl:hasOBONamespace>GAZ</oboInOwl:hasOBONamespace>
        <oboInOwl:id>GAZ:00058647</oboInOwl:id>
        <rdfs:label>Hope Arm</rdfs:label>
    </owl:NamedIndividual>
    


    <!-- http://purl.obolibrary.org/obo/GAZ_00058648 -->

    <owl:NamedIndividual rdf:about="http://purl.obolibrary.org/obo/GAZ_00058648">
        <rdf:type rdf:resource="http://purl.obolibrary.org/obo/ENVO_00000475"/>
        <obo:RO_0001025 rdf:resource="http://purl.obolibrary.org/obo/GAZ_00047041"/>
        <obo:IAO_0000115>An arm of Lake Manapouri.</obo:IAO_0000115>
        <oboInOwl:hasOBONamespace>GAZ</oboInOwl:hasOBONamespace>
        <oboInOwl:id>GAZ:00058648</oboInOwl:id>
        <rdfs:label>South Arm</rdfs:label>
    </owl:NamedIndividual>
    


    <!-- http://purl.obolibrary.org/obo/GAZ_00058649 -->

    <owl:NamedIndividual rdf:about="http://purl.obolibrary.org/obo/GAZ_00058649">
        <rdf:type rdf:resource="http://purl.obolibrary.org/obo/ENVO_00000475"/>
        <obo:RO_0001025 rdf:resource="http://purl.obolibrary.org/obo/GAZ_00047041"/>
        <obo:IAO_0000115>An arm of Lake Manapouri.</obo:IAO_0000115>
        <oboInOwl:hasOBONamespace>GAZ</oboInOwl:hasOBONamespace>
        <oboInOwl:id>GAZ:00058649</oboInOwl:id>
        <rdfs:label>North Arm</rdfs:label>
    </owl:NamedIndividual>
    


    <!-- http://purl.obolibrary.org/obo/GAZ_00058650 -->

    <owl:NamedIndividual rdf:about="http://purl.obolibrary.org/obo/GAZ_00058650">
        <rdf:type rdf:resource="http://purl.obolibrary.org/obo/ENVO_00000475"/>
        <obo:RO_0001025 rdf:resource="http://purl.obolibrary.org/obo/GAZ_00047041"/>
        <obo:IAO_0000115>An arm of Lake Manapouri.</obo:IAO_0000115>
        <oboInOwl:hasOBONamespace>GAZ</oboInOwl:hasOBONamespace>
        <oboInOwl:id>GAZ:00058650</oboInOwl:id>
        <rdfs:label>West Arm</rdfs:label>
    </owl:NamedIndividual>
    


    <!-- http://purl.obolibrary.org/obo/GAZ_00058651 -->

    <owl:NamedIndividual rdf:about="http://purl.obolibrary.org/obo/GAZ_00058651">
        <obo:RO_0001025 rdf:resource="http://purl.obolibrary.org/obo/GAZ_00047047"/>
        <obo:IAO_0000115>A lake in the southern part of Fiordland National Park, in New Zealand&apos;s South Island, 120 km northwest of Invercargill. It is drained in the northeast by the short Monowai River, which enters the Waiau River eight km to the northeast.</obo:IAO_0000115>
        <oboInOwl:hasOBONamespace>GAZ</oboInOwl:hasOBONamespace>
        <oboInOwl:id>GAZ:00058651</oboInOwl:id>
        <rdfs:label>Lake Monowai</rdfs:label>
    </owl:NamedIndividual>
    


    <!-- http://purl.obolibrary.org/obo/GAZ_00058652 -->

    <owl:NamedIndividual rdf:about="http://purl.obolibrary.org/obo/GAZ_00058652">
        <obo:RO_0001025 rdf:resource="http://purl.obolibrary.org/obo/GAZ_00047047"/>
        <obo:IAO_0000115>A lake located in a mountain valley in Fiordland National Park in the South Island of New Zealand. It is 35 km northwest of Tuatapere, between the similarly-sized lakes Monowai and Poteriteri. It drains via the 20 km-long Wairaurahiri River into Foveaux Strait 10 km to the west of Te Waewae Bay.</obo:IAO_0000115>
        <oboInOwl:hasOBONamespace>GAZ</oboInOwl:hasOBONamespace>
        <oboInOwl:id>GAZ:00058652</oboInOwl:id>
        <rdfs:label>Lake Hauroko</rdfs:label>
    </owl:NamedIndividual>
    


    <!-- http://purl.obolibrary.org/obo/GAZ_00058653 -->

    <owl:NamedIndividual rdf:about="http://purl.obolibrary.org/obo/GAZ_00058653">
        <obo:RO_0001025 rdf:resource="http://purl.obolibrary.org/obo/GAZ_00047047"/>
        <obo:IAO_0000115>A lake in Fiordland National Park in New Zealand&apos;s South Island. The outflow of Poteriteri is the Waitutu River, a short eight km river which flows into the western end of Foveaux Strait.</obo:IAO_0000115>
        <oboInOwl:hasOBONamespace>GAZ</oboInOwl:hasOBONamespace>
        <oboInOwl:id>GAZ:00058653</oboInOwl:id>
        <rdfs:label>Lake Poteriteri</rdfs:label>
    </owl:NamedIndividual>
    


    <!-- http://purl.obolibrary.org/obo/GAZ_00058654 -->

    <owl:NamedIndividual rdf:about="http://purl.obolibrary.org/obo/GAZ_00058654">
        <obo:RO_0001025 rdf:resource="http://purl.obolibrary.org/obo/GAZ_00008572"/>
        <obo:IAO_0000115>A geographic region of New Zealand that is situated on the south-western corner of the South Island. Most of it is covered by the Fiordland National Park.</obo:IAO_0000115>
        <oboInOwl:hasOBONamespace>GAZ</oboInOwl:hasOBONamespace>
        <oboInOwl:id>GAZ:00058654</oboInOwl:id>
        <rdfs:label>Fiordland</rdfs:label>
    </owl:NamedIndividual>
    


    <!-- http://purl.obolibrary.org/obo/GAZ_00058655 -->

    <owl:NamedIndividual rdf:about="http://purl.obolibrary.org/obo/GAZ_00058655">
        <obo:RO_0001025 rdf:resource="http://purl.obolibrary.org/obo/GAZ_00058654"/>
        <obo:IAO_0000115>A lake that lies at the northern end of Fiordland, in the southwest of New Zealand&apos;s South Island.</obo:IAO_0000115>
        <oboInOwl:hasOBONamespace>GAZ</oboInOwl:hasOBONamespace>
        <oboInOwl:id>GAZ:00058655</oboInOwl:id>
        <rdfs:label>Lake Alabaster</rdfs:label>
    </owl:NamedIndividual>
    


    <!-- http://purl.obolibrary.org/obo/GAZ_00058656 -->

    <owl:NamedIndividual rdf:about="http://purl.obolibrary.org/obo/GAZ_00058656">
        <obo:RO_0001025 rdf:resource="http://purl.obolibrary.org/obo/GAZ_00008572"/>
        <obo:IAO_0000115>A small lake at the eastern end of George Sound approximately 52 km north west of Te Anau in the Southland region of the South Island. The lake is fed by the Edith River and flows into George Sound via Alice Falls.</obo:IAO_0000115>
        <oboInOwl:hasOBONamespace>GAZ</oboInOwl:hasOBONamespace>
        <oboInOwl:id>GAZ:00058656</oboInOwl:id>
        <rdfs:label>Lake Alice</rdfs:label>
    </owl:NamedIndividual>
    


    <!-- http://purl.obolibrary.org/obo/GAZ_00058657 -->

    <owl:NamedIndividual rdf:about="http://purl.obolibrary.org/obo/GAZ_00058657">
        <obo:RO_0001025 rdf:resource="http://purl.obolibrary.org/obo/GAZ_00004772"/>
        <obo:IAO_0000115>A small lake approximately 7 km south west of Marton in the Manawatu-Wanganui region of the North Island.</obo:IAO_0000115>
        <oboInOwl:hasOBONamespace>GAZ</oboInOwl:hasOBONamespace>
        <oboInOwl:id>GAZ:00058657</oboInOwl:id>
        <rdfs:label>Lake Alice</rdfs:label>
    </owl:NamedIndividual>
    


    <!-- http://purl.obolibrary.org/obo/GAZ_00058658 -->

    <owl:NamedIndividual rdf:about="http://purl.obolibrary.org/obo/GAZ_00058658">
        <obo:RO_0001025 rdf:resource="http://purl.obolibrary.org/obo/GAZ_00004764"/>
        <obo:IAO_0000115>A mountain range and skifield in the South Island of New Zealand. Located on the southeastern shore of Lake Wakatipu.</obo:IAO_0000115>
        <oboInOwl:hasOBONamespace>GAZ</oboInOwl:hasOBONamespace>
        <oboInOwl:id>GAZ:00058658</oboInOwl:id>
        <rdfs:label>The Remarkables</rdfs:label>
    </owl:NamedIndividual>
    


    <!-- http://purl.obolibrary.org/obo/GAZ_00058659 -->

    <owl:NamedIndividual rdf:about="http://purl.obolibrary.org/obo/GAZ_00058659">
        <obo:RO_0001025 rdf:resource="http://purl.obolibrary.org/obo/GAZ_00058658"/>
        <obo:IAO_0000115>A lake located in The Remarkables near Queenstown in the South Island of New Zealand.</obo:IAO_0000115>
        <oboInOwl:hasOBONamespace>GAZ</oboInOwl:hasOBONamespace>
        <oboInOwl:id>GAZ:00058659</oboInOwl:id>
        <rdfs:label>Lake Alta</rdfs:label>
    </owl:NamedIndividual>
    


    <!-- http://purl.obolibrary.org/obo/GAZ_00058660 -->

    <owl:NamedIndividual rdf:about="http://purl.obolibrary.org/obo/GAZ_00058660">
        <obo:RO_0001025 rdf:resource="http://purl.obolibrary.org/obo/GAZ_00029957"/>
        <obo:IAO_0000115>A suburb of Porirua City approximately 22 km north of Wellington in New Zealand.</obo:IAO_0000115>
        <oboInOwl:hasOBONamespace>GAZ</oboInOwl:hasOBONamespace>
        <oboInOwl:id>GAZ:00058660</oboInOwl:id>
        <rdfs:label>Papakowhai</rdfs:label>
    </owl:NamedIndividual>
    


    <!-- http://purl.obolibrary.org/obo/GAZ_00058661 -->

    <owl:NamedIndividual rdf:about="http://purl.obolibrary.org/obo/GAZ_00058661">
        <obo:RO_0001025 rdf:resource="http://purl.obolibrary.org/obo/GAZ_00058660"/>
        <obo:IAO_0000115>An artificial lagoon located between Porirua city centre and northern suburb Papakowhai in New Zealand. In the 1950s the Porirua Harbour section of the North Island Main Trunk Railway was straightened with a causeway that created three lagoons at Papakowhai. The lagoons were partly filled in when the Ministry of Works and Development realigned State Highway 1 inland of the railway. The Ministry and community groups then transformed the area around the central lagoon into a public park that opened in 1980.</obo:IAO_0000115>
        <oboInOwl:hasOBONamespace>GAZ</oboInOwl:hasOBONamespace>
        <oboInOwl:id>GAZ:00058661</oboInOwl:id>
        <rdfs:label>Aotea Lagoon</rdfs:label>
    </owl:NamedIndividual>
    


    <!-- http://purl.obolibrary.org/obo/GAZ_00058662 -->

    <owl:NamedIndividual rdf:about="http://purl.obolibrary.org/obo/GAZ_00058662">
        <obo:RO_0001025 rdf:resource="http://purl.obolibrary.org/obo/GAZ_00004765"/>
        <obo:IAO_0000115>A river in the North Island, it runs for 425 km from the eastern slopes of Mount Ruapehu, joining the Tongariro River system and discharging to Lake Taupo, New Zealand&apos;s largest lake. It drains Taupo at the lake&apos;s northeastern edge, creates the Huka Falls, then flows northwest, through the Waikato Plains. It empties into the Tasman Sea south of Auckland at Port Waikato. The river&apos;s main tributary is the Waipa River, which has its confluence with the Waikato at Ngaruawahia.</obo:IAO_0000115>
        <oboInOwl:hasOBONamespace>GAZ</oboInOwl:hasOBONamespace>
        <oboInOwl:id>GAZ:00058662</oboInOwl:id>
        <rdfs:label>Waikato River</rdfs:label>
    </owl:NamedIndividual>
    


    <!-- http://purl.obolibrary.org/obo/GAZ_00058663 -->

    <owl:NamedIndividual rdf:about="http://purl.obolibrary.org/obo/GAZ_00058663">
        <obo:RO_0001025 rdf:resource="http://purl.obolibrary.org/obo/GAZ_00058662"/>
        <obo:IAO_0000115>An artificial lake formed as part of a hydroelectricity scheme on the Waikato River in the North Island of New Zealand. It is located 65 km southeast of Hamilton, to the north of Mangakino.</obo:IAO_0000115>
        <oboInOwl:hasOBONamespace>GAZ</oboInOwl:hasOBONamespace>
        <oboInOwl:id>GAZ:00058663</oboInOwl:id>
        <rdfs:label>Lake Arapuni</rdfs:label>
    </owl:NamedIndividual>
    


    <!-- http://purl.obolibrary.org/obo/GAZ_00058664 -->

    <owl:NamedIndividual rdf:about="http://purl.obolibrary.org/obo/GAZ_00058664">
        <obo:RO_0001025 rdf:resource="http://purl.obolibrary.org/obo/GAZ_00030225"/>
        <obo:IAO_0000115>An artificial lake in New Zealand&apos;s South Island, part of the Waitaki hydroelectric scheme. Immediately upstream is Lake Benmore and downstream Lake Waitaki.</obo:IAO_0000115>
        <oboInOwl:hasOBONamespace>GAZ</oboInOwl:hasOBONamespace>
        <oboInOwl:id>GAZ:00058664</oboInOwl:id>
        <rdfs:label>Lake Aviemore</rdfs:label>
    </owl:NamedIndividual>
    


    <!-- http://purl.obolibrary.org/obo/GAZ_00058665 -->

    <owl:NamedIndividual rdf:about="http://purl.obolibrary.org/obo/GAZ_00058665">
        <obo:RO_0001025 rdf:resource="http://purl.obolibrary.org/obo/GAZ_00030225"/>
        <obo:IAO_0000115>A lake located in the South Island of New Zealand. It was artificially created in the 1960s by construction of Benmore Dam. The major rivers with which it is fed are the Ohau, Pukaki and the Tekapo Rivers. Immediately downstream is Lake Aviemore.</obo:IAO_0000115>
        <oboInOwl:hasOBONamespace>GAZ</oboInOwl:hasOBONamespace>
        <oboInOwl:id>GAZ:00058665</oboInOwl:id>
        <rdfs:label>Lake Benmore</rdfs:label>
    </owl:NamedIndividual>
    


    <!-- http://purl.obolibrary.org/obo/GAZ_00058666 -->

    <owl:NamedIndividual rdf:about="http://purl.obolibrary.org/obo/GAZ_00058666">
        <obo:RO_0001025 rdf:resource="http://purl.obolibrary.org/obo/GAZ_00008562"/>
        <obo:IAO_0000115>A small lake at the foot of the Tasman Glacier in inland Canterbury, in the cental South Island of New Zealand. Its outflow is the Tasman River, part of the Waitaki River system.</obo:IAO_0000115>
        <oboInOwl:hasOBONamespace>GAZ</oboInOwl:hasOBONamespace>
        <oboInOwl:id>GAZ:00058666</oboInOwl:id>
        <rdfs:label>Blue Lake</rdfs:label>
    </owl:NamedIndividual>
    


    <!-- http://purl.obolibrary.org/obo/GAZ_00058667 -->

    <owl:NamedIndividual rdf:about="http://purl.obolibrary.org/obo/GAZ_00058667">
        <obo:RO_0001025 rdf:resource="http://purl.obolibrary.org/obo/GAZ_00008563"/>
        <obo:IAO_0000115>A national park located in the South Island of New Zealand.</obo:IAO_0000115>
        <oboInOwl:hasOBONamespace>GAZ</oboInOwl:hasOBONamespace>
        <oboInOwl:id>GAZ:00058667</oboInOwl:id>
        <rdfs:label>Nelson Lakes National Park</rdfs:label>
    </owl:NamedIndividual>
    


    <!-- http://purl.obolibrary.org/obo/GAZ_00058668 -->

    <owl:NamedIndividual rdf:about="http://purl.obolibrary.org/obo/GAZ_00058668">
        <obo:RO_0001025 rdf:resource="http://purl.obolibrary.org/obo/GAZ_00008563"/>
        <obo:RO_0001025 rdf:resource="http://purl.obolibrary.org/obo/GAZ_00058667"/>
        <obo:IAO_0000115>A mountain lake within the borders of the Nelson Lakes National Park. It is fed by the Travers River. The water from the lake flows into the Buller River.</obo:IAO_0000115>
        <oboInOwl:hasOBONamespace>GAZ</oboInOwl:hasOBONamespace>
        <oboInOwl:id>GAZ:00058668</oboInOwl:id>
        <rdfs:label>Lake Rotoiti</rdfs:label>
    </owl:NamedIndividual>
    


    <!-- http://purl.obolibrary.org/obo/GAZ_00058669 -->

    <owl:NamedIndividual rdf:about="http://purl.obolibrary.org/obo/GAZ_00058669">
        <obo:RO_0001025 rdf:resource="http://purl.obolibrary.org/obo/GAZ_00058667"/>
        <obo:IAO_0000115>A lake located within the borders of Nelson Lakes National Park in the South Island. The lake is fed by the D&apos;Urville and Sabine rivers.</obo:IAO_0000115>
        <oboInOwl:hasOBONamespace>GAZ</oboInOwl:hasOBONamespace>
        <oboInOwl:id>GAZ:00058669</oboInOwl:id>
        <rdfs:label>Lake Rotoroa</rdfs:label>
    </owl:NamedIndividual>
    


    <!-- http://purl.obolibrary.org/obo/GAZ_00058670 -->

    <owl:NamedIndividual rdf:about="http://purl.obolibrary.org/obo/GAZ_00058670">
        <obo:RO_0001025 rdf:resource="http://purl.obolibrary.org/obo/GAZ_00058667"/>
        <obo:IAO_0000115>A tiny lake in Nelson Lakes National Park, in the northern reaches of the Southern Alps. It is drained by the Sabine River, which is part of the Buller River system. It is fed from Lake Constance by an underground segment of the Sabine.</obo:IAO_0000115>
        <oboInOwl:hasOBONamespace>GAZ</oboInOwl:hasOBONamespace>
        <oboInOwl:id>GAZ:00058670</oboInOwl:id>
        <rdfs:label>Blue Lake</rdfs:label>
    </owl:NamedIndividual>
    


    <!-- http://purl.obolibrary.org/obo/GAZ_00058671 -->

    <owl:NamedIndividual rdf:about="http://purl.obolibrary.org/obo/GAZ_00058671">
        <obo:RO_0001025 rdf:resource="http://purl.obolibrary.org/obo/GAZ_00058667"/>
        <obo:IAO_0000115>An alpine lake in the South Island of New Zealand. It lies within the borders of the Nelson Lakes National Park. The lake is drained via an underground river into Blue Lake.</obo:IAO_0000115>
        <oboInOwl:hasOBONamespace>GAZ</oboInOwl:hasOBONamespace>
        <oboInOwl:id>GAZ:00058671</oboInOwl:id>
        <rdfs:label>Lake Constance</rdfs:label>
    </owl:NamedIndividual>
    


    <!-- http://purl.obolibrary.org/obo/GAZ_00058672 -->

    <owl:NamedIndividual rdf:about="http://purl.obolibrary.org/obo/GAZ_00058672">
        <obo:RO_0001025 rdf:resource="http://purl.obolibrary.org/obo/GAZ_00004767"/>
        <obo:IAO_0000115>A small artificial lake adjacent to the town of Saint Bathans is in the Central Otago region of the South Island of New Zealand. It is the result of sluicing operations that began in 1873 when John Ewing (1844-1922) formed the Saint Bathans Channel Company to mine the Kildare Hill Gold Claim in St Bathans.</obo:IAO_0000115>
        <oboInOwl:hasOBONamespace>GAZ</oboInOwl:hasOBONamespace>
        <oboInOwl:id>GAZ:00058672</oboInOwl:id>
        <rdfs:label>Blue Lake</rdfs:label>
    </owl:NamedIndividual>
    


    <!-- http://purl.obolibrary.org/obo/GAZ_00058673 -->

    <owl:NamedIndividual rdf:about="http://purl.obolibrary.org/obo/GAZ_00058673">
        <obo:RO_0001025 rdf:resource="http://purl.obolibrary.org/obo/GAZ_00004764"/>
        <obo:IAO_0000115>A lake in NW South Island of New Zealand, covering an area of 40 km2. The lake&apos;s outflow is the Arnold River, a tributary of the Grey River. The lake lies 31 km to the southeast of Greymouth.</obo:IAO_0000115>
        <oboInOwl:hasOBONamespace>GAZ</oboInOwl:hasOBONamespace>
        <oboInOwl:id>GAZ:00058673</oboInOwl:id>
        <rdfs:label>Lake Brunner</rdfs:label>
    </owl:NamedIndividual>
    


    <!-- http://purl.obolibrary.org/obo/GAZ_00058674 -->

    <owl:NamedIndividual rdf:about="http://purl.obolibrary.org/obo/GAZ_00058674">
        <obo:RO_0001025 rdf:resource="http://purl.obolibrary.org/obo/GAZ_00004764"/>
        <obo:IAO_0000115>A small lake in the north of New Zealand&apos;s South Island. It is located 12 km southwest of the Lewis Pass. The lake is the source of the Grey River.</obo:IAO_0000115>
        <oboInOwl:hasOBONamespace>GAZ</oboInOwl:hasOBONamespace>
        <oboInOwl:id>GAZ:00058674</oboInOwl:id>
        <rdfs:label>Lake Christabel</rdfs:label>
    </owl:NamedIndividual>
    


    <!-- http://purl.obolibrary.org/obo/GAZ_00058675 -->

    <owl:NamedIndividual rdf:about="http://purl.obolibrary.org/obo/GAZ_00058675">
        <obo:RO_0001025 rdf:resource="http://purl.obolibrary.org/obo/GAZ_00008562"/>
        <obo:IAO_0000115>A lake located 35 km to the northwest of Methven, in inland Canterbury, in New Zealand&apos;s South Island. The lake is located to the north of the Rakaia River, and is the site of one of the country&apos;s earliest hydroelectric schemes, completed in 1914. The project makes use of the difference in altitude between the lake and river (the lake is 150 metres higher). Both the Harper and Wilberforce Rivers have had some of their flow diverted into the lake.</obo:IAO_0000115>
        <oboInOwl:hasOBONamespace>GAZ</oboInOwl:hasOBONamespace>
        <oboInOwl:id>GAZ:00058675</oboInOwl:id>
        <rdfs:label>Lake Coleridge</rdfs:label>
    </owl:NamedIndividual>
    


    <!-- http://purl.obolibrary.org/obo/GAZ_00058676 -->

    <owl:NamedIndividual rdf:about="http://purl.obolibrary.org/obo/GAZ_00058676">
        <obo:RO_0001025 rdf:resource="http://purl.obolibrary.org/obo/GAZ_00008563"/>
        <obo:IAO_0000115>A lake in the Tasman District of the South Island of New Zealand. It is drained by Frazer Stream which in turn feeds into the Alfred River.</obo:IAO_0000115>
        <oboInOwl:hasOBONamespace>GAZ</oboInOwl:hasOBONamespace>
        <oboInOwl:id>GAZ:00058676</oboInOwl:id>
        <rdfs:label>Lake Daniell</rdfs:label>
    </owl:NamedIndividual>
    


    <!-- http://purl.obolibrary.org/obo/GAZ_00058677 -->

    <owl:NamedIndividual rdf:about="http://purl.obolibrary.org/obo/GAZ_00058677">
        <obo:RO_0001025 rdf:resource="http://purl.obolibrary.org/obo/GAZ_00004767"/>
        <obo:IAO_0000115>A lake located in the Central Otago region of New Zealand. It is fed by the Hunter River. Lake Hawea is dammed to the south by an ancient terminal moraine created some 10,000 years ago.</obo:IAO_0000115>
        <oboInOwl:hasOBONamespace>GAZ</oboInOwl:hasOBONamespace>
        <oboInOwl:id>GAZ:00058677</oboInOwl:id>
        <rdfs:label>Lake Hawea</rdfs:label>
    </owl:NamedIndividual>
    


    <!-- http://purl.obolibrary.org/obo/GAZ_00058678 -->

    <owl:NamedIndividual rdf:about="http://purl.obolibrary.org/obo/GAZ_00058678">
        <obo:RO_0001025 rdf:resource="http://purl.obolibrary.org/obo/GAZ_00047062"/>
        <obo:IAO_0000115>An artificial lake, created by the Roxburgh Dam on the Clutha River, some 160 km from Dunedin.</obo:IAO_0000115>
        <oboInOwl:hasOBONamespace>GAZ</oboInOwl:hasOBONamespace>
        <oboInOwl:id>GAZ:00058678</oboInOwl:id>
        <rdfs:label>Lake Roxburgh</rdfs:label>
    </owl:NamedIndividual>
    


    <!-- http://purl.obolibrary.org/obo/GAZ_00058679 -->

    <owl:NamedIndividual rdf:about="http://purl.obolibrary.org/obo/GAZ_00058679">
        <obo:RO_0001025 rdf:resource="http://purl.obolibrary.org/obo/GAZ_00004767"/>
        <obo:IAO_0000115>A small lake in South Otago, in the South Island of New Zealand. It is located to the northeast of Balclutha, close to the small town of Kaitangata.</obo:IAO_0000115>
        <oboInOwl:hasOBONamespace>GAZ</oboInOwl:hasOBONamespace>
        <oboInOwl:id>GAZ:00058679</oboInOwl:id>
        <rdfs:label>Lake Tuakitoto</rdfs:label>
    </owl:NamedIndividual>
    


    <!-- http://purl.obolibrary.org/obo/GAZ_00058680 -->

    <owl:NamedIndividual rdf:about="http://purl.obolibrary.org/obo/GAZ_00058680">
        <obo:RO_0001025 rdf:resource="http://purl.obolibrary.org/obo/GAZ_00004767"/>
        <obo:IAO_0000115>A tidal freshwater lake located 15 km north of Milton in Otago, in New Zealand&apos;s South Island. Waihola is drained by the Waipori River, a tributary of the Taieri.</obo:IAO_0000115>
        <oboInOwl:hasOBONamespace>GAZ</oboInOwl:hasOBONamespace>
        <oboInOwl:id>GAZ:00058680</oboInOwl:id>
        <rdfs:label>Lake Waihola</rdfs:label>
    </owl:NamedIndividual>
    


    <!-- http://purl.obolibrary.org/obo/GAZ_00058681 -->

    <owl:NamedIndividual rdf:about="http://purl.obolibrary.org/obo/GAZ_00058681">
        <obo:RO_0001025 rdf:resource="http://purl.obolibrary.org/obo/GAZ_00004767"/>
        <obo:IAO_0000115>A lake located in the wetlands to the south west of Dunedin in New Zealand on the Waipori River. The Waipori River is a major tributary of the Taieri River, and these wetlands form the southern edge of the Taieri Plains.</obo:IAO_0000115>
        <oboInOwl:hasOBONamespace>GAZ</oboInOwl:hasOBONamespace>
        <oboInOwl:id>GAZ:00058681</oboInOwl:id>
        <rdfs:label>Lake Waipori</rdfs:label>
    </owl:NamedIndividual>
    


    <!-- http://purl.obolibrary.org/obo/GAZ_00058682 -->

    <owl:NamedIndividual rdf:about="http://purl.obolibrary.org/obo/GAZ_00058682">
        <obo:RO_0001025 rdf:resource="http://purl.obolibrary.org/obo/GAZ_00047062"/>
        <obo:IAO_0000115>A lake located in the South Island of New Zealand. The lake was formed on the Clutha River as a result of the construction of the Clyde Dam during the 1990s.</obo:IAO_0000115>
        <oboInOwl:hasOBONamespace>GAZ</oboInOwl:hasOBONamespace>
        <oboInOwl:id>GAZ:00058682</oboInOwl:id>
        <rdfs:label>Lake Dunstan</rdfs:label>
    </owl:NamedIndividual>
    


    <!-- http://purl.obolibrary.org/obo/GAZ_00058683 -->

    <owl:NamedIndividual rdf:about="http://purl.obolibrary.org/obo/GAZ_00058683">
        <obo:RO_0001025 rdf:resource="http://purl.obolibrary.org/obo/GAZ_00008562"/>
        <obo:IAO_0000115>A lake located in the Canterbury region of the South Island of New Zealand. It is a broad, shallow lake located directly to the west of Banks Peninsula, separated from the Pacific Ocean by a long narrow strip of land called Kaitorete Spit.</obo:IAO_0000115>
        <oboInOwl:hasOBONamespace>GAZ</oboInOwl:hasOBONamespace>
        <oboInOwl:id>GAZ:00058683</oboInOwl:id>
        <rdfs:label>Lake Ellesmere</rdfs:label>
    </owl:NamedIndividual>
    


    <!-- http://purl.obolibrary.org/obo/GAZ_00058684 -->

    <owl:NamedIndividual rdf:about="http://purl.obolibrary.org/obo/GAZ_00058684">
        <obo:RO_0001025 rdf:resource="http://purl.obolibrary.org/obo/GAZ_00008562"/>
        <obo:IAO_0000115>A long finger of land which extends along the coast of Canterbury in the South Island of New Zealand. It runs southwest from Banks Peninsula for 25 km, and separates the shallow Lake Ellesmere from the Canterbury Bight and Pacific Ocean.</obo:IAO_0000115>
        <oboInOwl:hasOBONamespace>GAZ</oboInOwl:hasOBONamespace>
        <oboInOwl:id>GAZ:00058684</oboInOwl:id>
        <rdfs:label>Kaitorete Spit</rdfs:label>
    </owl:NamedIndividual>
    


    <!-- http://purl.obolibrary.org/obo/GAZ_00058685 -->

    <owl:NamedIndividual rdf:about="http://purl.obolibrary.org/obo/GAZ_00058685">
        <obo:RO_0001025 rdf:resource="http://purl.obolibrary.org/obo/GAZ_00004764"/>
        <obo:IAO_0000115>A lake close to Cook Strait in the northeastern South Island of New Zealand. It is 25 miles south of Blenheim and 6 miles south of the mouth of the Awatere River, is a shallow lagoon protected from the open sea by a single barrier beach covered by sand dunes. It is on the north-easterly extension of the Ward depression.</obo:IAO_0000115>
        <oboInOwl:hasOBONamespace>GAZ</oboInOwl:hasOBONamespace>
        <oboInOwl:id>GAZ:00058685</oboInOwl:id>
        <rdfs:label>Lake Grassmere</rdfs:label>
    </owl:NamedIndividual>
    


    <!-- http://purl.obolibrary.org/obo/GAZ_00058686 -->

    <owl:NamedIndividual rdf:about="http://purl.obolibrary.org/obo/GAZ_00058686">
        <obo:RO_0001025 rdf:resource="http://purl.obolibrary.org/obo/GAZ_00058687"/>
        <obo:IAO_0000115>A lake lying between Lake Rotorua and Lake Tarawera in the Bay of Plenty region of New Zealand&apos;s North Island.</obo:IAO_0000115>
        <oboInOwl:hasOBONamespace>GAZ</oboInOwl:hasOBONamespace>
        <oboInOwl:id>GAZ:00058686</oboInOwl:id>
        <rdfs:label>Lake Rotokakahi</rdfs:label>
    </owl:NamedIndividual>
    


    <!-- http://purl.obolibrary.org/obo/GAZ_00058687 -->

    <owl:NamedIndividual rdf:about="http://purl.obolibrary.org/obo/GAZ_00058687">
        <obo:RO_0001025 rdf:resource="http://purl.obolibrary.org/obo/GAZ_00007723"/>
        <obo:RO_0001025 rdf:resource="http://purl.obolibrary.org/obo/GAZ_00053845"/>
        <oboInOwl:hasOBONamespace>GAZ</oboInOwl:hasOBONamespace>
        <oboInOwl:id>GAZ:00058687</oboInOwl:id>
        <rdfs:label>Okataina Caldera</rdfs:label>
    </owl:NamedIndividual>
    


    <!-- http://purl.obolibrary.org/obo/GAZ_00058688 -->

    <owl:NamedIndividual rdf:about="http://purl.obolibrary.org/obo/GAZ_00058688">
        <obo:RO_0001025 rdf:resource="http://purl.obolibrary.org/obo/GAZ_00058687"/>
        <obo:IAO_0000115>A lake lying between Lake Rotorua and Lake Tarawera in the Bay of Plenty region of New Zealand&apos;s North Island.</obo:IAO_0000115>
        <oboInOwl:hasOBONamespace>GAZ</oboInOwl:hasOBONamespace>
        <oboInOwl:id>GAZ:00058688</oboInOwl:id>
        <rdfs:label>Lake Tikitapu</rdfs:label>
    </owl:NamedIndividual>
    


    <!-- http://purl.obolibrary.org/obo/GAZ_00058689 -->

    <owl:NamedIndividual rdf:about="http://purl.obolibrary.org/obo/GAZ_00058689">
        <obo:RO_0001025 rdf:resource="http://purl.obolibrary.org/obo/GAZ_00058687"/>
        <obo:IAO_0000115>A lake lying between Lake Rotorua and Lake Tarawera in the Bay of Plenty region of New Zealand&apos;s North Island.</obo:IAO_0000115>
        <oboInOwl:hasOBONamespace>GAZ</oboInOwl:hasOBONamespace>
        <oboInOwl:id>GAZ:00058689</oboInOwl:id>
        <rdfs:label>Lake Okareka</rdfs:label>
    </owl:NamedIndividual>
    


    <!-- http://purl.obolibrary.org/obo/GAZ_00058690 -->

    <owl:NamedIndividual rdf:about="http://purl.obolibrary.org/obo/GAZ_00058690">
        <obo:RO_0001025 rdf:resource="http://purl.obolibrary.org/obo/GAZ_00058687"/>
        <obo:IAO_0000115>A lake lying between Lake Rotorua and Lake Tarawera in the Bay of Plenty region of New Zealand&apos;s North Island.</obo:IAO_0000115>
        <oboInOwl:hasOBONamespace>GAZ</oboInOwl:hasOBONamespace>
        <oboInOwl:id>GAZ:00058690</oboInOwl:id>
        <rdfs:label>Lake Okataina</rdfs:label>
    </owl:NamedIndividual>
    


    <!-- http://purl.obolibrary.org/obo/GAZ_00058691 -->

    <owl:NamedIndividual rdf:about="http://purl.obolibrary.org/obo/GAZ_00058691">
        <obo:RO_0001025 rdf:resource="http://purl.obolibrary.org/obo/GAZ_00058687"/>
        <obo:IAO_0000115>A lake that lies within the Okataina caldera. It is located 18 km to the east of Rotorua, and five km to the west of Mount Tarawera. The lake is filled primarily by sources from the nearby Blue (Lake Tikitapu) and Green (Lake Rotokakahi) lakes.</obo:IAO_0000115>
        <oboInOwl:hasOBONamespace>GAZ</oboInOwl:hasOBONamespace>
        <oboInOwl:id>GAZ:00058691</oboInOwl:id>
        <rdfs:label>Lake Tarawera</rdfs:label>
    </owl:NamedIndividual>
    


    <!-- http://purl.obolibrary.org/obo/GAZ_00058692 -->

    <owl:NamedIndividual rdf:about="http://purl.obolibrary.org/obo/GAZ_00058692">
        <obo:RO_0001025 rdf:resource="http://purl.obolibrary.org/obo/GAZ_00058654"/>
        <obo:IAO_0000115>A small lake, which is a 3 hour walk tramp in from the Borland Road.</obo:IAO_0000115>
        <oboInOwl:hasOBONamespace>GAZ</oboInOwl:hasOBONamespace>
        <oboInOwl:id>GAZ:00058692</oboInOwl:id>
        <rdfs:label>Green Lake</rdfs:label>
    </owl:NamedIndividual>
    


    <!-- http://purl.obolibrary.org/obo/GAZ_00058693 -->

    <owl:NamedIndividual rdf:about="http://purl.obolibrary.org/obo/GAZ_00058693">
        <obo:RO_0001025 rdf:resource="http://purl.obolibrary.org/obo/GAZ_00047047"/>
        <obo:IAO_0000115>A lake in the South Island of New Zealand, located between Lake Te Anau and Milford Sound, it lies close to the State Highway 94 (the Milford Sound Road).</obo:IAO_0000115>
        <oboInOwl:hasOBONamespace>GAZ</oboInOwl:hasOBONamespace>
        <oboInOwl:id>GAZ:00058693</oboInOwl:id>
        <rdfs:label>Lake Gunn</rdfs:label>
    </owl:NamedIndividual>
    


    <!-- http://purl.obolibrary.org/obo/GAZ_00058694 -->

    <owl:NamedIndividual rdf:about="http://purl.obolibrary.org/obo/GAZ_00058694">
        <obo:RO_0001025 rdf:resource="http://purl.obolibrary.org/obo/GAZ_00009539"/>
        <obo:IAO_0000115>A small lake in Central Otago, in New Zealand&apos;s South Island. It is located close to the towns of Arrowtown and Queenstown.</obo:IAO_0000115>
        <oboInOwl:hasOBONamespace>GAZ</oboInOwl:hasOBONamespace>
        <oboInOwl:id>GAZ:00058694</oboInOwl:id>
        <rdfs:label>Lake Hayes</rdfs:label>
    </owl:NamedIndividual>
    


    <!-- http://purl.obolibrary.org/obo/GAZ_00058695 -->

    <owl:NamedIndividual rdf:about="http://purl.obolibrary.org/obo/GAZ_00058695">
        <rdf:type rdf:resource="http://purl.obolibrary.org/obo/ENVO_00000856"/>
        <obo:RO_0001025 rdf:resource="http://purl.obolibrary.org/obo/GAZ_00010244"/>
        <obo:IAO_0000115>A populated place. A town in Canterbury, New Zealand, now little more than a suburb of Ashburton. It lies to the south of the larger town, separated from it by the Ashburton River.</obo:IAO_0000115>
        <oboInOwl:hasOBONamespace>GAZ</oboInOwl:hasOBONamespace>
        <oboInOwl:id>GAZ:00058695</oboInOwl:id>
        <rdfs:label>Tinwald</rdfs:label>
    </owl:NamedIndividual>
    


    <!-- http://purl.obolibrary.org/obo/GAZ_00058696 -->

    <owl:NamedIndividual rdf:about="http://purl.obolibrary.org/obo/GAZ_00058696">
        <obo:RO_0001025 rdf:resource="http://purl.obolibrary.org/obo/GAZ_00010244"/>
        <obo:IAO_0000115>An artificial recreational lake, located 6 km south-east of Tinwald in the locality of Huntingdon, Canterbury, New Zealand.</obo:IAO_0000115>
        <oboInOwl:hasOBONamespace>GAZ</oboInOwl:hasOBONamespace>
        <oboInOwl:id>GAZ:00058696</oboInOwl:id>
        <rdfs:label>Lake Hood</rdfs:label>
    </owl:NamedIndividual>
    


    <!-- http://purl.obolibrary.org/obo/GAZ_00058697 -->

    <owl:NamedIndividual rdf:about="http://purl.obolibrary.org/obo/GAZ_00058697">
        <obo:RO_0001025 rdf:resource="http://purl.obolibrary.org/obo/GAZ_00029952"/>
        <obo:IAO_0000115>A lake located in the Horowhenua, an area of the southern Manawatu-Wanganui region in New Zealand&apos;s North Island. It lies on a sandy plain two km to the west of Levin and five km from the coast of the Tasman Sea. It is a shallow lake, only some two metres in depth, fed by various small streams, and is drained by the Hokio Stream.</obo:IAO_0000115>
        <oboInOwl:hasOBONamespace>GAZ</oboInOwl:hasOBONamespace>
        <oboInOwl:id>GAZ:00058697</oboInOwl:id>
        <rdfs:label>Lake Horowhenua</rdfs:label>
    </owl:NamedIndividual>
    


    <!-- http://purl.obolibrary.org/obo/GAZ_00058698 -->

    <owl:NamedIndividual rdf:about="http://purl.obolibrary.org/obo/GAZ_00058698">
        <obo:RO_0001025 rdf:resource="http://purl.obolibrary.org/obo/GAZ_00010256"/>
        <obo:IAO_0000115>A small lake approximately 14 km east of Waipawa in the Hawke&apos;s Bay region of the North Island of New Zealand.</obo:IAO_0000115>
        <oboInOwl:hasOBONamespace>GAZ</oboInOwl:hasOBONamespace>
        <oboInOwl:id>GAZ:00058698</oboInOwl:id>
        <rdfs:label>Horseshoe Lake</rdfs:label>
    </owl:NamedIndividual>
    


    <!-- http://purl.obolibrary.org/obo/GAZ_00058699 -->

    <owl:NamedIndividual rdf:about="http://purl.obolibrary.org/obo/GAZ_00058699">
        <obo:RO_0001025 rdf:resource="http://purl.obolibrary.org/obo/GAZ_00008561"/>
        <obo:IAO_0000115>A small lake in the western outskirts of Hamilton in the Waikato region of the North Island of New Zealand.</obo:IAO_0000115>
        <oboInOwl:hasOBONamespace>GAZ</oboInOwl:hasOBONamespace>
        <oboInOwl:id>GAZ:00058699</oboInOwl:id>
        <rdfs:label>Horseshoe Lake</rdfs:label>
    </owl:NamedIndividual>
    


    <!-- http://purl.obolibrary.org/obo/GAZ_00058700 -->

    <owl:NamedIndividual rdf:about="http://purl.obolibrary.org/obo/GAZ_00058700">
        <obo:RO_0001025 rdf:resource="http://purl.obolibrary.org/obo/GAZ_00010246"/>
        <obo:IAO_0000115>A small urban lake in northeast Christchurch, close to the Avon River.</obo:IAO_0000115>
        <oboInOwl:hasOBONamespace>GAZ</oboInOwl:hasOBONamespace>
        <oboInOwl:id>GAZ:00058700</oboInOwl:id>
        <rdfs:label>Horseshoe Lake</rdfs:label>
    </owl:NamedIndividual>
    


    <!-- http://purl.obolibrary.org/obo/GAZ_00058701 -->

    <owl:NamedIndividual rdf:about="http://purl.obolibrary.org/obo/GAZ_00058701">
        <obo:RO_0001025 rdf:resource="http://purl.obolibrary.org/obo/GAZ_00008562"/>
        <obo:IAO_0000115>A small lake approximately 27km south west of Hanmer Springs in the Canterbury region of the South Island of New Zealand.</obo:IAO_0000115>
        <oboInOwl:hasOBONamespace>GAZ</oboInOwl:hasOBONamespace>
        <oboInOwl:id>GAZ:00058701</oboInOwl:id>
        <rdfs:label>Horseshoe Lake</rdfs:label>
    </owl:NamedIndividual>
    


    <!-- http://purl.obolibrary.org/obo/GAZ_00058702 -->

    <owl:NamedIndividual rdf:about="http://purl.obolibrary.org/obo/GAZ_00058702">
        <obo:RO_0001025 rdf:resource="http://purl.obolibrary.org/obo/GAZ_00004777"/>
        <obo:IAO_0000115>A lake located on the West Coast of New Zealand&apos;s South Island. A number of small streams flow into the lake and it empties into the Wanganui River. It is close to the coast and near the rural settlements of Pukekura and Harihari, and State Highway 6 runs along the eastern shore of the lake on its route between Ross and the Franz Josef Glacier.</obo:IAO_0000115>
        <oboInOwl:hasOBONamespace>GAZ</oboInOwl:hasOBONamespace>
        <oboInOwl:id>GAZ:00058702</oboInOwl:id>
        <rdfs:label>Lake Ianthe</rdfs:label>
    </owl:NamedIndividual>
    


    <!-- http://purl.obolibrary.org/obo/GAZ_00058703 -->

    <owl:NamedIndividual rdf:about="http://purl.obolibrary.org/obo/GAZ_00058703">
        <obo:RO_0001025 rdf:resource="http://purl.obolibrary.org/obo/GAZ_00004764"/>
        <obo:IAO_0000115>A river in the South Island of New Zealand. The river flows out of Lake Innes and into the sea on the southern coast of the South Island.</obo:IAO_0000115>
        <oboInOwl:hasOBONamespace>GAZ</oboInOwl:hasOBONamespace>
        <oboInOwl:id>GAZ:00058703</oboInOwl:id>
        <rdfs:label>Aan River</rdfs:label>
    </owl:NamedIndividual>
    


    <!-- http://purl.obolibrary.org/obo/GAZ_00058704 -->

    <owl:NamedIndividual rdf:about="http://purl.obolibrary.org/obo/GAZ_00058704">
        <obo:RO_0001025 rdf:resource="http://purl.obolibrary.org/obo/GAZ_00004764"/>
        <obo:RO_0001025 rdf:resource="http://purl.obolibrary.org/obo/GAZ_00058703"/>
        <obo:IAO_0000115>A lake in the South Island of New Zealand. The source of the Aan River.</obo:IAO_0000115>
        <oboInOwl:hasOBONamespace>GAZ</oboInOwl:hasOBONamespace>
        <oboInOwl:id>GAZ:00058704</oboInOwl:id>
        <rdfs:label>Lake Innes</rdfs:label>
    </owl:NamedIndividual>
    


    <!-- http://purl.obolibrary.org/obo/GAZ_00058705 -->

    <owl:NamedIndividual rdf:about="http://purl.obolibrary.org/obo/GAZ_00058705">
        <obo:RO_0001025 rdf:resource="http://purl.obolibrary.org/obo/GAZ_00004777"/>
        <obo:IAO_0000115>A lake located on the West Coast of New Zealand&apos;s South Island. It lies 30 km southeast of Hokitika, and drains into the Tasman Sea via the Kaniere and Hokitika rivers.</obo:IAO_0000115>
        <oboInOwl:hasOBONamespace>GAZ</oboInOwl:hasOBONamespace>
        <oboInOwl:id>GAZ:00058705</oboInOwl:id>
        <rdfs:label>Lake Kaniere</rdfs:label>
    </owl:NamedIndividual>
    


    <!-- http://purl.obolibrary.org/obo/GAZ_00058706 -->

    <owl:NamedIndividual rdf:about="http://purl.obolibrary.org/obo/GAZ_00058706">
        <obo:RO_0001025 rdf:resource="http://purl.obolibrary.org/obo/GAZ_00058662"/>
        <obo:IAO_0000115>An artificial lake formed as part of a hydroelectricity scheme on the Waikato River in the North Island of New Zealand. It is located 35 km southeast of Hamilton, close to the town of Cambridge.</obo:IAO_0000115>
        <oboInOwl:hasOBONamespace>GAZ</oboInOwl:hasOBONamespace>
        <oboInOwl:id>GAZ:00058706</oboInOwl:id>
        <rdfs:label>Lake Karapiro</rdfs:label>
    </owl:NamedIndividual>
    


    <!-- http://purl.obolibrary.org/obo/GAZ_00058707 -->

    <owl:NamedIndividual rdf:about="http://purl.obolibrary.org/obo/GAZ_00058707">
        <obo:RO_0001025 rdf:resource="http://purl.obolibrary.org/obo/GAZ_00058708"/>
        <obo:IAO_0000115>A lake located to the east of Pencarrow Head, on the eastern side of New Zealand&apos;s Wellington Harbour, in East Harbour Regional Park, and is fed by Cameron Stream which rises on private land to its north.</obo:IAO_0000115>
        <oboInOwl:hasOBONamespace>GAZ</oboInOwl:hasOBONamespace>
        <oboInOwl:id>GAZ:00058707</oboInOwl:id>
        <rdfs:label>Lake Kohangapiripiri</rdfs:label>
    </owl:NamedIndividual>
    


    <!-- http://purl.obolibrary.org/obo/GAZ_00058708 -->

    <owl:NamedIndividual rdf:about="http://purl.obolibrary.org/obo/GAZ_00058708">
        <obo:RO_0001025 rdf:resource="http://purl.obolibrary.org/obo/GAZ_00008565"/>
        <obo:IAO_0000115>Two freshwater Pencarrow lakes in Fitzroy Bay which formed in valleys which became blocked to the nearby sea after earthquakes changed the topography.</obo:IAO_0000115>
        <oboInOwl:hasOBONamespace>GAZ</oboInOwl:hasOBONamespace>
        <oboInOwl:id>GAZ:00058708</oboInOwl:id>
        <rdfs:label>Pencarrow Lakes</rdfs:label>
    </owl:NamedIndividual>
    


    <!-- http://purl.obolibrary.org/obo/GAZ_00058709 -->

    <owl:NamedIndividual rdf:about="http://purl.obolibrary.org/obo/GAZ_00058709">
        <obo:RO_0001025 rdf:resource="http://purl.obolibrary.org/obo/GAZ_00058708"/>
        <obo:IAO_0000115>A lake located to the east of Pencarrow Head, on the eastern side of New Zealand&apos;s Wellington Harbour, in East Harbour Regional Park. It is fed by Gollans Stream, which has its headwaters on Mount Lowry, 14 km to the north.</obo:IAO_0000115>
        <oboInOwl:hasOBONamespace>GAZ</oboInOwl:hasOBONamespace>
        <oboInOwl:id>GAZ:00058709</oboInOwl:id>
        <rdfs:label>Lake Kohangatera</rdfs:label>
    </owl:NamedIndividual>
    


    <!-- http://purl.obolibrary.org/obo/GAZ_00058710 -->

    <owl:NamedIndividual rdf:about="http://purl.obolibrary.org/obo/GAZ_00058710">
        <obo:RO_0001025 rdf:resource="http://purl.obolibrary.org/obo/GAZ_00058662"/>
        <obo:IAO_0000115>An artificial lake of the Waikato river system in New Zealand. It was created through the building of the Ohakuri hydroelectric power station in 1961.</obo:IAO_0000115>
        <oboInOwl:hasOBONamespace>GAZ</oboInOwl:hasOBONamespace>
        <oboInOwl:id>GAZ:00058710</oboInOwl:id>
        <rdfs:label>Lake Ohakuri</rdfs:label>
    </owl:NamedIndividual>
    


    <!-- http://purl.obolibrary.org/obo/GAZ_00058711 -->

    <owl:NamedIndividual rdf:about="http://purl.obolibrary.org/obo/GAZ_00058711">
        <obo:RO_0001025 rdf:resource="http://purl.obolibrary.org/obo/GAZ_00004760"/>
        <obo:IAO_0000115>A chain of hills generally running approximately 25 km from north to south generally 25 km west of central Auckland, New Zealand.</obo:IAO_0000115>
        <oboInOwl:hasOBONamespace>GAZ</oboInOwl:hasOBONamespace>
        <oboInOwl:id>GAZ:00058711</oboInOwl:id>
        <rdfs:label>Waitakere Ranges</rdfs:label>
    </owl:NamedIndividual>
    


    <!-- http://purl.obolibrary.org/obo/GAZ_00058712 -->

    <owl:NamedIndividual rdf:about="http://purl.obolibrary.org/obo/GAZ_00058712">
        <obo:RO_0001025 rdf:resource="http://purl.obolibrary.org/obo/GAZ_00058711"/>
        <obo:IAO_0000115>A reservoir in the Waitakere Ranges that supplies water to Auckland. Completed in 1948.</obo:IAO_0000115>
        <oboInOwl:hasOBONamespace>GAZ</oboInOwl:hasOBONamespace>
        <oboInOwl:id>GAZ:00058712</oboInOwl:id>
        <rdfs:label>Lower Nihotupu Reservoir</rdfs:label>
    </owl:NamedIndividual>
    


    <!-- http://purl.obolibrary.org/obo/GAZ_00058713 -->

    <owl:NamedIndividual rdf:about="http://purl.obolibrary.org/obo/GAZ_00058713">
        <obo:RO_0001025 rdf:resource="http://purl.obolibrary.org/obo/GAZ_00008562"/>
        <obo:IAO_0000115>A small lake in the Canterbury region of New Zealand&apos;s South Island. It is near Porters Pass, and State Highway 73 from Springfield and Cass skirts the lake&apos;s northeastern shore.</obo:IAO_0000115>
        <oboInOwl:hasOBONamespace>GAZ</oboInOwl:hasOBONamespace>
        <oboInOwl:id>GAZ:00058713</oboInOwl:id>
        <rdfs:label>Lake Lyndon</rdfs:label>
    </owl:NamedIndividual>
    


    <!-- http://purl.obolibrary.org/obo/GAZ_00058714 -->

    <owl:NamedIndividual rdf:about="http://purl.obolibrary.org/obo/GAZ_00058714">
        <obo:RO_0001025 rdf:resource="http://purl.obolibrary.org/obo/GAZ_00004777"/>
        <obo:IAO_0000115>A shallow lake on the West Coast of New Zealand&apos;s South Island. It is roughly 10 km south of Hokitika and near the small town of Ruatapu. It was formerly a coastal lagoon, but the buildup of coastal dunes made it an inland lake roughly 500 m from the Tasman Sea coastline.</obo:IAO_0000115>
        <oboInOwl:hasOBONamespace>GAZ</oboInOwl:hasOBONamespace>
        <oboInOwl:id>GAZ:00058714</oboInOwl:id>
        <rdfs:label>Lake Mahinapua</rdfs:label>
    </owl:NamedIndividual>
    


    <!-- http://purl.obolibrary.org/obo/GAZ_00058715 -->

    <owl:NamedIndividual rdf:about="http://purl.obolibrary.org/obo/GAZ_00058715">
        <obo:RO_0001025 rdf:resource="http://purl.obolibrary.org/obo/GAZ_00004767"/>
        <obo:IAO_0000115>A river located in Otago in the South Island of New Zealand. Rising in the Lammerlaw Range, it flows southeast for 50 km before joining the Taieri River near Henley, 30 km southwest of Dunedin of which it is officially the southernmost border.</obo:IAO_0000115>
        <oboInOwl:hasOBONamespace>GAZ</oboInOwl:hasOBONamespace>
        <oboInOwl:id>GAZ:00058715</oboInOwl:id>
        <rdfs:label>Waipori River</rdfs:label>
    </owl:NamedIndividual>
    


    <!-- http://purl.obolibrary.org/obo/GAZ_00058716 -->

    <owl:NamedIndividual rdf:about="http://purl.obolibrary.org/obo/GAZ_00058716">
        <obo:RO_0001025 rdf:resource="http://purl.obolibrary.org/obo/GAZ_00058715"/>
        <obo:IAO_0000115>A small reservoir formed by a dam on the Waipori River 35 km to the west of Dunedin in New Zealand&apos;s South Island. It lies on the western side of Maungatua, above and to the west of the Berwick Forest.</obo:IAO_0000115>
        <oboInOwl:hasOBONamespace>GAZ</oboInOwl:hasOBONamespace>
        <oboInOwl:id>GAZ:00058716</oboInOwl:id>
        <rdfs:label>Lake Mahinerangi</rdfs:label>
    </owl:NamedIndividual>
    


    <!-- http://purl.obolibrary.org/obo/GAZ_00058717 -->

    <owl:NamedIndividual rdf:about="http://purl.obolibrary.org/obo/GAZ_00058717">
        <obo:RO_0001025 rdf:resource="http://purl.obolibrary.org/obo/GAZ_00004777"/>
        <obo:IAO_0000115>A lake located in the West Coast of New Zealand&apos;s South Island. It lies north of Franz Josef Glacier, and drains into the Okarito Lagoon.</obo:IAO_0000115>
        <oboInOwl:hasOBONamespace>GAZ</oboInOwl:hasOBONamespace>
        <oboInOwl:id>GAZ:00058717</oboInOwl:id>
        <rdfs:label>Lake Mapourika</rdfs:label>
    </owl:NamedIndividual>
    


    <!-- http://purl.obolibrary.org/obo/GAZ_00058719 -->

    <owl:NamedIndividual rdf:about="http://purl.obolibrary.org/obo/GAZ_00058719">
        <obo:RO_0001025 rdf:resource="http://purl.obolibrary.org/obo/GAZ_00058662"/>
        <obo:IAO_0000115>A reservoir formed as part of a hydroelectricity scheme on the Waikato River in the North Island of New Zealand. It is located 85 km southeast of Hamilton, close to the town of Mangakino.</obo:IAO_0000115>
        <oboInOwl:hasOBONamespace>GAZ</oboInOwl:hasOBONamespace>
        <oboInOwl:id>GAZ:00058719</oboInOwl:id>
        <rdfs:label>Lake Maraetai</rdfs:label>
    </owl:NamedIndividual>
    


    <!-- http://purl.obolibrary.org/obo/GAZ_00058720 -->

    <owl:NamedIndividual rdf:about="http://purl.obolibrary.org/obo/GAZ_00058720">
        <obo:RO_0001025 rdf:resource="http://purl.obolibrary.org/obo/GAZ_00058721"/>
        <obo:IAO_0000115>A lake in the Darran Mountains in the Fiordland National Park in the South Island of New Zealand. It is fed and drained by Marian Creek which in turn feeds into the Hollyford River.</obo:IAO_0000115>
        <oboInOwl:hasOBONamespace>GAZ</oboInOwl:hasOBONamespace>
        <oboInOwl:id>GAZ:00058720</oboInOwl:id>
        <rdfs:label>Lake Marian</rdfs:label>
    </owl:NamedIndividual>
    


    <!-- http://purl.obolibrary.org/obo/GAZ_00058721 -->

    <owl:NamedIndividual rdf:about="http://purl.obolibrary.org/obo/GAZ_00058721">
        <obo:RO_0001025 rdf:resource="http://purl.obolibrary.org/obo/GAZ_00047047"/>
        <oboInOwl:hasOBONamespace>GAZ</oboInOwl:hasOBONamespace>
        <oboInOwl:id>GAZ:00058721</oboInOwl:id>
        <rdfs:label>Darran Mountains</rdfs:label>
    </owl:NamedIndividual>
    


    <!-- http://purl.obolibrary.org/obo/GAZ_00058722 -->

    <owl:NamedIndividual rdf:about="http://purl.obolibrary.org/obo/GAZ_00058722">
        <obo:RO_0001025 rdf:resource="http://purl.obolibrary.org/obo/GAZ_00004778"/>
        <obo:RO_0001025 rdf:resource="http://purl.obolibrary.org/obo/GAZ_00030217"/>
        <obo:IAO_0000115>A lake located near the Fox Glacier in South Westland, New Zealand. It is situated on the valley floor about 12 km from the current Fox Glacier and Mount Cook.</obo:IAO_0000115>
        <oboInOwl:hasOBONamespace>GAZ</oboInOwl:hasOBONamespace>
        <oboInOwl:id>GAZ:00058722</oboInOwl:id>
        <rdfs:label>Lake Matheson</rdfs:label>
    </owl:NamedIndividual>
    


    <!-- http://purl.obolibrary.org/obo/GAZ_00058723 -->

    <owl:NamedIndividual rdf:about="http://purl.obolibrary.org/obo/GAZ_00058723">
        <obo:RO_0001025 rdf:resource="http://purl.obolibrary.org/obo/GAZ_00008563"/>
        <obo:IAO_0000115>A national park in the northwest of the South Island of New Zealand. It was gazetted in 1996. Kahurangi Point, regarded as the boundary between the West Coast and Tasman Regions, is located in the park, as are the Heaphy Track and Mount Owen.</obo:IAO_0000115>
        <oboInOwl:hasOBONamespace>GAZ</oboInOwl:hasOBONamespace>
        <oboInOwl:id>GAZ:00058723</oboInOwl:id>
        <rdfs:label>Kahurangi National Park</rdfs:label>
    </owl:NamedIndividual>
    


    <!-- http://purl.obolibrary.org/obo/GAZ_00058724 -->

    <owl:NamedIndividual rdf:about="http://purl.obolibrary.org/obo/GAZ_00058724">
        <rdf:type rdf:resource="http://purl.obolibrary.org/obo/ENVO_00000305"/>
        <obo:RO_0001025 rdf:resource="http://purl.obolibrary.org/obo/GAZ_00058723"/>
        <obo:IAO_0000115>A headland on the West Coast of New Zealand&apos;s South Island, overlooking the Tasman Sea. It is located in Kahurangi National Park between Karamea and Farewell Spit. Kahurangi Point is traditionally regarded as the northernmost point of the West Coast region, although for most purposes it is considered part of the Tasman/Nelson region.</obo:IAO_0000115>
        <oboInOwl:hasOBONamespace>GAZ</oboInOwl:hasOBONamespace>
        <oboInOwl:id>GAZ:00058724</oboInOwl:id>
        <rdfs:label>Kahurangi Point</rdfs:label>
    </owl:NamedIndividual>
    


    <!-- http://purl.obolibrary.org/obo/GAZ_00058725 -->

    <owl:NamedIndividual rdf:about="http://purl.obolibrary.org/obo/GAZ_00058725">
        <obo:RO_0001025 rdf:resource="http://purl.obolibrary.org/obo/GAZ_00058723"/>
        <obo:RO_0001025 rdf:resource="http://purl.obolibrary.org/obo/GAZ_00058726"/>
        <obo:IAO_0000115>A lake in Kahurangi National Park, in the North West corner of New Zealand&apos;s South Island.</obo:IAO_0000115>
        <oboInOwl:hasOBONamespace>GAZ</oboInOwl:hasOBONamespace>
        <oboInOwl:id>GAZ:00058725</oboInOwl:id>
        <rdfs:label>Lake Matiri</rdfs:label>
    </owl:NamedIndividual>
    


    <!-- http://purl.obolibrary.org/obo/GAZ_00058726 -->

    <owl:NamedIndividual rdf:about="http://purl.obolibrary.org/obo/GAZ_00058726">
        <obo:RO_0001025 rdf:resource="http://purl.obolibrary.org/obo/GAZ_00004764"/>
        <obo:IAO_0000115>A small river located in the northwest of New Zealand&apos;s South Island. It runs south for 30 km from its headwaters west of Mount Owen in Kahurangi National Park to its confluence with the Buller River just below the town of Murchison. Halfway along its length, it passes through Lake Matiri.</obo:IAO_0000115>
        <oboInOwl:hasOBONamespace>GAZ</oboInOwl:hasOBONamespace>
        <oboInOwl:id>GAZ:00058726</oboInOwl:id>
        <rdfs:label>Matiri River</rdfs:label>
    </owl:NamedIndividual>
    


    <!-- http://purl.obolibrary.org/obo/GAZ_00058727 -->

    <owl:NamedIndividual rdf:about="http://purl.obolibrary.org/obo/GAZ_00058727">
        <obo:RO_0001025 rdf:resource="http://purl.obolibrary.org/obo/GAZ_00004764"/>
        <obo:IAO_0000115>Two lakes located in the South Island of New Zealand.</obo:IAO_0000115>
        <oboInOwl:hasOBONamespace>GAZ</oboInOwl:hasOBONamespace>
        <oboInOwl:id>GAZ:00058727</oboInOwl:id>
        <rdfs:label>Mavora Lakes</rdfs:label>
    </owl:NamedIndividual>
    


    <!-- http://purl.obolibrary.org/obo/GAZ_00058728 -->

    <owl:NamedIndividual rdf:about="http://purl.obolibrary.org/obo/GAZ_00058728">
        <obo:RO_0001025 rdf:resource="http://purl.obolibrary.org/obo/GAZ_00058727"/>
        <obo:IAO_0000115>One of the Mavora Lakes.</obo:IAO_0000115>
        <oboInOwl:hasOBONamespace>GAZ</oboInOwl:hasOBONamespace>
        <oboInOwl:id>GAZ:00058728</oboInOwl:id>
        <rdfs:label>North Mavora Lake</rdfs:label>
    </owl:NamedIndividual>
    


    <!-- http://purl.obolibrary.org/obo/GAZ_00058729 -->

    <owl:NamedIndividual rdf:about="http://purl.obolibrary.org/obo/GAZ_00058729">
        <obo:RO_0001025 rdf:resource="http://purl.obolibrary.org/obo/GAZ_00058727"/>
        <obo:IAO_0000115>One of the Mavora Lakes.</obo:IAO_0000115>
        <oboInOwl:hasOBONamespace>GAZ</oboInOwl:hasOBONamespace>
        <oboInOwl:id>GAZ:00058729</oboInOwl:id>
        <rdfs:label>South Mavora Lake</rdfs:label>
    </owl:NamedIndividual>
    


    <!-- http://purl.obolibrary.org/obo/GAZ_00058730 -->

    <owl:NamedIndividual rdf:about="http://purl.obolibrary.org/obo/GAZ_00058730">
        <obo:RO_0001025 rdf:resource="http://purl.obolibrary.org/obo/GAZ_00058654"/>
        <obo:IAO_0000115>A lake that lies at the northern end of Fiordland, in the southwest of New Zealand&apos;s South Island. Lake McKerrow drains, and is drained by, the Hollyford River. The lake is technically a fiord which has been cut off from the Tasman Sea by sediment. The sea is now three km from the lake&apos;s northern end.</obo:IAO_0000115>
        <oboInOwl:hasOBONamespace>GAZ</oboInOwl:hasOBONamespace>
        <oboInOwl:id>GAZ:00058730</oboInOwl:id>
        <rdfs:label>Lake McKerrow</rdfs:label>
    </owl:NamedIndividual>
    


    <!-- http://purl.obolibrary.org/obo/GAZ_00058731 -->

    <owl:NamedIndividual rdf:about="http://purl.obolibrary.org/obo/GAZ_00058731">
        <obo:RO_0001025 rdf:resource="http://purl.obolibrary.org/obo/GAZ_00058732"/>
        <obo:IAO_0000115>A small lake located with the New Zealand Army&apos;s Waiouru Training area. It is fed by tributaries running off the slopes of Mt Ruapehu, and feeds water into the Tongariro River Hydro scheme via the Moawhango Tunnel. The lake is dammed at the southern end.</obo:IAO_0000115>
        <oboInOwl:hasOBONamespace>GAZ</oboInOwl:hasOBONamespace>
        <oboInOwl:id>GAZ:00058731</oboInOwl:id>
        <rdfs:label>Lake Moawhango</rdfs:label>
    </owl:NamedIndividual>
    


    <!-- http://purl.obolibrary.org/obo/GAZ_00058732 -->

    <owl:NamedIndividual rdf:about="http://purl.obolibrary.org/obo/GAZ_00058732">
        <obo:RO_0001025 rdf:resource="http://purl.obolibrary.org/obo/GAZ_00004765"/>
        <obo:IAO_0000115>A training area for the New Zealand Army.</obo:IAO_0000115>
        <oboInOwl:hasOBONamespace>GAZ</oboInOwl:hasOBONamespace>
        <oboInOwl:id>GAZ:00058732</oboInOwl:id>
        <rdfs:label>Waiouru Training Area</rdfs:label>
    </owl:NamedIndividual>
    


    <!-- http://purl.obolibrary.org/obo/GAZ_00058733 -->

    <owl:NamedIndividual rdf:about="http://purl.obolibrary.org/obo/GAZ_00058733">
        <obo:RO_0001025 rdf:resource="http://purl.obolibrary.org/obo/GAZ_00010256"/>
        <obo:IAO_0000115>A small lake located to the northwest of the city of Hastings in the Hawke&apos;s Bay Region of the eastern North Island of New Zealand.</obo:IAO_0000115>
        <oboInOwl:hasOBONamespace>GAZ</oboInOwl:hasOBONamespace>
        <oboInOwl:id>GAZ:00058733</oboInOwl:id>
        <rdfs:label>Lake Oingo</rdfs:label>
    </owl:NamedIndividual>
    


    <!-- http://purl.obolibrary.org/obo/GAZ_00058734 -->

    <owl:NamedIndividual rdf:about="http://purl.obolibrary.org/obo/GAZ_00058734">
        <obo:RO_0001025 rdf:resource="http://purl.obolibrary.org/obo/GAZ_00008569"/>
        <obo:IAO_0000115>A small lake in the Northland Region of New Zealand. It is located just to the north of the town of Kaikohe.</obo:IAO_0000115>
        <oboInOwl:hasOBONamespace>GAZ</oboInOwl:hasOBONamespace>
        <oboInOwl:id>GAZ:00058734</oboInOwl:id>
        <rdfs:label>Lake Omapere</rdfs:label>
    </owl:NamedIndividual>
    


    <!-- http://purl.obolibrary.org/obo/GAZ_00058735 -->

    <owl:NamedIndividual rdf:about="http://purl.obolibrary.org/obo/GAZ_00058735">
        <obo:RO_0001025 rdf:resource="http://purl.obolibrary.org/obo/GAZ_00004777"/>
        <obo:IAO_0000115>A small lake 30 km north of Haast on the West Coast of New Zealand&apos;s South Island. It is close to State Highway 6, six km inland from the coast of the Tasman Sea. The lake is drained at its northern end by a small stream which joins the Paringa River. The Paringa River flows into the Tasman Sea eight km north of the lake.</obo:IAO_0000115>
        <oboInOwl:hasOBONamespace>GAZ</oboInOwl:hasOBONamespace>
        <oboInOwl:id>GAZ:00058735</oboInOwl:id>
        <rdfs:label>Lake Paringa</rdfs:label>
    </owl:NamedIndividual>
    


    <!-- http://purl.obolibrary.org/obo/GAZ_00058736 -->

    <owl:NamedIndividual rdf:about="http://purl.obolibrary.org/obo/GAZ_00058736">
        <obo:RO_0001025 rdf:resource="http://purl.obolibrary.org/obo/GAZ_00004777"/>
        <obo:IAO_0000115>A shallow lake located in the West Coast region of New Zealand&apos;s South Island roughly 13 km southeast from Lake Brunner. A number of small streams flow into the lake, and the Poerua River flows from the lake into the Crooked River, which leads to Lake Brunner.</obo:IAO_0000115>
        <oboInOwl:hasOBONamespace>GAZ</oboInOwl:hasOBONamespace>
        <oboInOwl:id>GAZ:00058736</oboInOwl:id>
        <rdfs:label>Lake Poerua</rdfs:label>
    </owl:NamedIndividual>
    


    <!-- http://purl.obolibrary.org/obo/GAZ_00058737 -->

    <owl:NamedIndividual rdf:about="http://purl.obolibrary.org/obo/GAZ_00058737">
        <obo:RO_0001025 rdf:resource="http://purl.obolibrary.org/obo/GAZ_00010256"/>
        <obo:IAO_0000115>A small shallow hardwater lake in the Hawke&apos;s Bay Region, North Island,New Zealand. It is located about 20 km south-west of Hastings, New Zealand and 150 km south-east of the Taupo Volcanic Zone, close to the settlement of Te Hauke. It was deeper in the past (about 2.5 m) but it became articifially drained after the 1931 Hawke&apos;s Bay earthquake.</obo:IAO_0000115>
        <oboInOwl:hasOBONamespace>GAZ</oboInOwl:hasOBONamespace>
        <oboInOwl:id>GAZ:00058737</oboInOwl:id>
        <rdfs:label>Lake Poukawa</rdfs:label>
    </owl:NamedIndividual>
    


    <!-- http://purl.obolibrary.org/obo/GAZ_00058738 -->

    <owl:NamedIndividual rdf:about="http://purl.obolibrary.org/obo/GAZ_00058738">
        <obo:RO_0001025 rdf:resource="http://purl.obolibrary.org/obo/GAZ_00053838"/>
        <obo:IAO_0000115>A freshwater lake occupying a volcanic explosion crater between the suburbs of Takapuna and Milford on the North Shore of Auckland, New Zealand. Separated from the sea by less than 200 m at one point, it has a circumference of about 4.5 km and reaches 57 m in depth.</obo:IAO_0000115>
        <oboInOwl:hasOBONamespace>GAZ</oboInOwl:hasOBONamespace>
        <oboInOwl:id>GAZ:00058738</oboInOwl:id>
        <rdfs:label>Lake Pupuke</rdfs:label>
    </owl:NamedIndividual>
    


    <!-- http://purl.obolibrary.org/obo/GAZ_00058739 -->

    <owl:NamedIndividual rdf:about="http://purl.obolibrary.org/obo/GAZ_00058739">
        <obo:RO_0001025 rdf:resource="http://purl.obolibrary.org/obo/GAZ_00007723"/>
        <obo:IAO_0000115>A small lake in northern New Zealand, located 30 km to the east of Rotorua. It is immediately south of the active volcano Mount Tarawera, and its geography was substantially altered by a major eruption in 1886.</obo:IAO_0000115>
        <oboInOwl:hasOBONamespace>GAZ</oboInOwl:hasOBONamespace>
        <oboInOwl:id>GAZ:00058739</oboInOwl:id>
        <rdfs:label>Lake Rerewhakaaitu</rdfs:label>
    </owl:NamedIndividual>
    


    <!-- http://purl.obolibrary.org/obo/GAZ_00058740 -->

    <owl:NamedIndividual rdf:about="http://purl.obolibrary.org/obo/GAZ_00058740">
        <obo:RO_0001025 rdf:resource="http://purl.obolibrary.org/obo/GAZ_00009541"/>
        <obo:IAO_0000115>A small lake to the south of Lake Taupo on the North Island Volcanic Plateau in New Zealand. The lake is located in a graben between the broad volcanic dome of Mount Tongariro to the south and the smaller volcanic peak of Pihanga to the northewst. It is naturally drained by the Pouto Stream into the Tongariro River.</obo:IAO_0000115>
        <oboInOwl:hasOBONamespace>GAZ</oboInOwl:hasOBONamespace>
        <oboInOwl:id>GAZ:00058740</oboInOwl:id>
        <rdfs:label>Lake Rotoaira</rdfs:label>
    </owl:NamedIndividual>
    


    <!-- http://purl.obolibrary.org/obo/GAZ_00058741 -->

    <owl:NamedIndividual rdf:about="http://purl.obolibrary.org/obo/GAZ_00058741">
        <obo:RO_0001025 rdf:resource="http://purl.obolibrary.org/obo/GAZ_00058687"/>
        <obo:IAO_0000115>The smallest in a chain of three lakes to the northeast of Lake Rotorua in New Zealand&apos;s North Island. It is located between the city of Rotorua and town of Whakatane. The southern end of the lake occupies part of the Okataina caldera. It is fed by Lake Rotoma to the east, and flows westward joining Lake Rotoiti.</obo:IAO_0000115>
        <oboInOwl:hasOBONamespace>GAZ</oboInOwl:hasOBONamespace>
        <oboInOwl:id>GAZ:00058741</oboInOwl:id>
        <rdfs:label>Lake Rotoehu</rdfs:label>
    </owl:NamedIndividual>
    


    <!-- http://purl.obolibrary.org/obo/GAZ_00058742 -->

    <owl:NamedIndividual rdf:about="http://purl.obolibrary.org/obo/GAZ_00058742">
        <obo:RO_0001025 rdf:resource="http://purl.obolibrary.org/obo/GAZ_00058687"/>
        <obo:IAO_0000115>The northwesternmost in a chain of lakes formed within the Okataina caldera. It drains to the Kaituna River, which flows into the Bay of Plenty near Maketu.</obo:IAO_0000115>
        <oboInOwl:hasOBONamespace>GAZ</oboInOwl:hasOBONamespace>
        <oboInOwl:id>GAZ:00058742</oboInOwl:id>
        <rdfs:label>Lake Rotoiti</rdfs:label>
    </owl:NamedIndividual>
    


    <!-- http://purl.obolibrary.org/obo/GAZ_00058743 -->

    <owl:NamedIndividual rdf:about="http://purl.obolibrary.org/obo/GAZ_00058743">
        <obo:RO_0001025 rdf:resource="http://purl.obolibrary.org/obo/GAZ_00058687"/>
        <obo:IAO_0000115>The easternmost in a chain of three lakes to the northeast of Lake Rotorua in New Zealand&apos;s North Island. Like the others, it lies within the Okataina caldera. It is located exactly half-way between the city of Rotorua and town of Whakatane.</obo:IAO_0000115>
        <oboInOwl:hasOBONamespace>GAZ</oboInOwl:hasOBONamespace>
        <oboInOwl:id>GAZ:00058743</oboInOwl:id>
        <rdfs:label>Lake Rotoma</rdfs:label>
    </owl:NamedIndividual>
    


    <!-- http://purl.obolibrary.org/obo/GAZ_00058744 -->

    <owl:NamedIndividual rdf:about="http://purl.obolibrary.org/obo/GAZ_00058744">
        <obo:RO_0001025 rdf:resource="http://purl.obolibrary.org/obo/GAZ_00053849"/>
        <obo:RO_0001025 rdf:resource="http://purl.obolibrary.org/obo/GAZ_00058687"/>
        <obo:IAO_0000115>A small lake in northern New Zealand, located 25 km to the east of Rotorua. It is immediately southwest of the dormant volcano Mount Tarawera, and its geography was substantially altered by a major eruption in 1886. Along with the mountain, it lies within the Okataina caldera.</obo:IAO_0000115>
        <oboInOwl:hasOBONamespace>GAZ</oboInOwl:hasOBONamespace>
        <oboInOwl:id>GAZ:00058744</oboInOwl:id>
        <rdfs:label>Lake Rotomahana</rdfs:label>
    </owl:NamedIndividual>
    


    <!-- http://purl.obolibrary.org/obo/GAZ_00058745 -->

    <owl:NamedIndividual rdf:about="http://purl.obolibrary.org/obo/GAZ_00058745">
        <obo:RO_0001025 rdf:resource="http://purl.obolibrary.org/obo/GAZ_00007545"/>
        <obo:IAO_0000115>A crater lake in the Pihanga Scenic Reserve, in the Tongariro National Park in New Zealand&apos;s Central North Island. It lies at the North West foot of Mount Pihanga.</obo:IAO_0000115>
        <oboInOwl:hasOBONamespace>GAZ</oboInOwl:hasOBONamespace>
        <oboInOwl:id>GAZ:00058745</oboInOwl:id>
        <rdfs:label>Lake Rotopounamu</rdfs:label>
    </owl:NamedIndividual>
    


    <!-- http://purl.obolibrary.org/obo/GAZ_00058746 -->

    <owl:NamedIndividual rdf:about="http://purl.obolibrary.org/obo/GAZ_00058746">
        <obo:RO_0001025 rdf:resource="http://purl.obolibrary.org/obo/GAZ_00008561"/>
        <obo:IAO_0000115>A lake in Hamilton, Waikato, New Zealand.</obo:IAO_0000115>
        <oboInOwl:hasOBONamespace>GAZ</oboInOwl:hasOBONamespace>
        <oboInOwl:id>GAZ:00058746</oboInOwl:id>
        <rdfs:label>Lake Rotoroa</rdfs:label>
    </owl:NamedIndividual>
    


    <!-- http://purl.obolibrary.org/obo/GAZ_00058747 -->

    <owl:NamedIndividual rdf:about="http://purl.obolibrary.org/obo/GAZ_00058747">
        <obo:RO_0001025 rdf:resource="http://purl.obolibrary.org/obo/GAZ_00047054"/>
        <obo:IAO_0000115>A reservoir located in the Mackenzie Basin in New Zealand&apos;s South Island. An artificial lake, it was formed as part of the Waitaki hydroelectric project. The Ohau River flows into the lake, which lies on the traditional boundary of the Canterbury and Otago regions.</obo:IAO_0000115>
        <oboInOwl:hasOBONamespace>GAZ</oboInOwl:hasOBONamespace>
        <oboInOwl:id>GAZ:00058747</oboInOwl:id>
        <rdfs:label>Lake Ruataniwha</rdfs:label>
    </owl:NamedIndividual>
    


    <!-- http://purl.obolibrary.org/obo/GAZ_00058748 -->

    <owl:NamedIndividual rdf:about="http://purl.obolibrary.org/obo/GAZ_00058748">
        <obo:RO_0001025 rdf:resource="http://purl.obolibrary.org/obo/GAZ_00010256"/>
        <obo:IAO_0000115>A small lake located to the west of the city of Hastings in the Hawke&apos;s Bay Region of the eastern North Island of New Zealand.</obo:IAO_0000115>
        <oboInOwl:hasOBONamespace>GAZ</oboInOwl:hasOBONamespace>
        <oboInOwl:id>GAZ:00058748</oboInOwl:id>
        <rdfs:label>Lake Runanga</rdfs:label>
    </owl:NamedIndividual>
    


    <!-- http://purl.obolibrary.org/obo/GAZ_00058749 -->

    <owl:NamedIndividual rdf:about="http://purl.obolibrary.org/obo/GAZ_00058749">
        <obo:RO_0001025 rdf:resource="http://purl.obolibrary.org/obo/GAZ_00004777"/>
        <obo:IAO_0000115>A lagoon located on the West Coast of New Zealand&apos;s South Island. It is in the southern Westland District, with Abut Head to the west and the village of Harihari to the east/southeast. The lagoon is located on the coast of the Tasman Sea and has a narrow sea opening at the western end that lets in saltwater. No rivers feed into the lagoon, but the Hinatua River passes very close to the lagoon&apos;s eastern shore.</obo:IAO_0000115>
        <oboInOwl:hasOBONamespace>GAZ</oboInOwl:hasOBONamespace>
        <oboInOwl:id>GAZ:00058749</oboInOwl:id>
        <rdfs:label>Saltwater Lagoon</rdfs:label>
    </owl:NamedIndividual>
    


    <!-- http://purl.obolibrary.org/obo/GAZ_00058750 -->

    <owl:NamedIndividual rdf:about="http://purl.obolibrary.org/obo/GAZ_00058750">
        <obo:RO_0001025 rdf:resource="http://purl.obolibrary.org/obo/GAZ_00008562"/>
        <obo:IAO_0000115>A portected Area in Canterbury Region.</obo:IAO_0000115>
        <oboInOwl:hasOBONamespace>GAZ</oboInOwl:hasOBONamespace>
        <oboInOwl:id>GAZ:00058750</oboInOwl:id>
        <rdfs:label>Lake Sumner Forest Park</rdfs:label>
    </owl:NamedIndividual>
    


    <!-- http://purl.obolibrary.org/obo/GAZ_00058751 -->

    <owl:NamedIndividual rdf:about="http://purl.obolibrary.org/obo/GAZ_00058751">
        <obo:RO_0001025 rdf:resource="http://purl.obolibrary.org/obo/GAZ_00058750"/>
        <obo:IAO_0000115>A lake situated 100 km northwest of Christchurch, Canterbury. The lake is located in the Lake Sumner Forest Park.</obo:IAO_0000115>
        <oboInOwl:hasOBONamespace>GAZ</oboInOwl:hasOBONamespace>
        <oboInOwl:id>GAZ:00058751</oboInOwl:id>
        <rdfs:label>Lake Sumner</rdfs:label>
    </owl:NamedIndividual>
    


    <!-- http://purl.obolibrary.org/obo/GAZ_00058752 -->

    <owl:NamedIndividual rdf:about="http://purl.obolibrary.org/obo/GAZ_00058752">
        <obo:RO_0001025 rdf:resource="http://purl.obolibrary.org/obo/GAZ_00058750"/>
        <obo:IAO_0000115>A lake in Lake Sumner Forest Park.</obo:IAO_0000115>
        <oboInOwl:hasOBONamespace>GAZ</oboInOwl:hasOBONamespace>
        <oboInOwl:id>GAZ:00058752</oboInOwl:id>
        <rdfs:label>Lake Taylor</rdfs:label>
    </owl:NamedIndividual>
    


    <!-- http://purl.obolibrary.org/obo/GAZ_00058753 -->

    <owl:NamedIndividual rdf:about="http://purl.obolibrary.org/obo/GAZ_00058753">
        <obo:RO_0001025 rdf:resource="http://purl.obolibrary.org/obo/GAZ_00058750"/>
        <obo:IAO_0000115>A lake in Lake Sumner Forest Park.</obo:IAO_0000115>
        <oboInOwl:hasOBONamespace>GAZ</oboInOwl:hasOBONamespace>
        <oboInOwl:id>GAZ:00058753</oboInOwl:id>
        <rdfs:label>Lake Mason</rdfs:label>
    </owl:NamedIndividual>
    


    <!-- http://purl.obolibrary.org/obo/GAZ_00058754 -->

    <owl:NamedIndividual rdf:about="http://purl.obolibrary.org/obo/GAZ_00058754">
        <obo:RO_0001025 rdf:resource="http://purl.obolibrary.org/obo/GAZ_00058750"/>
        <obo:IAO_0000115>A lake in Lake Sumner Forest Park.</obo:IAO_0000115>
        <oboInOwl:hasOBONamespace>GAZ</oboInOwl:hasOBONamespace>
        <oboInOwl:id>GAZ:00058754</oboInOwl:id>
        <rdfs:label>Lake Sheppard</rdfs:label>
    </owl:NamedIndividual>
    


    <!-- http://purl.obolibrary.org/obo/GAZ_00058755 -->

    <owl:NamedIndividual rdf:about="http://purl.obolibrary.org/obo/GAZ_00058755">
        <obo:RO_0001025 rdf:resource="http://purl.obolibrary.org/obo/GAZ_00058750"/>
        <obo:IAO_0000115>A lake in Lake Sumner Forest Park.</obo:IAO_0000115>
        <oboInOwl:hasOBONamespace>GAZ</oboInOwl:hasOBONamespace>
        <oboInOwl:id>GAZ:00058755</oboInOwl:id>
        <rdfs:label>Loch Katrine</rdfs:label>
    </owl:NamedIndividual>
    


    <!-- http://purl.obolibrary.org/obo/GAZ_00058757 -->

    <owl:NamedIndividual rdf:about="http://purl.obolibrary.org/obo/GAZ_00058757">
        <obo:RO_0001025 rdf:resource="http://purl.obolibrary.org/obo/GAZ_00016318"/>
        <obo:IAO_0000115>A lagoon on Chatham Island, in the South Pacific Ocean off New Zealand&apos;s east coast. It is the outflow of several small rivers in the island&apos;s hilly south, and drains to the Pacific via gaps in Hanson Bay on the island&apos;s east coast.</obo:IAO_0000115>
        <oboInOwl:hasOBONamespace>GAZ</oboInOwl:hasOBONamespace>
        <oboInOwl:id>GAZ:00058757</oboInOwl:id>
        <rdfs:label>Te Whanga Lagoon</rdfs:label>
    </owl:NamedIndividual>
    


    <!-- http://purl.obolibrary.org/obo/GAZ_00058759 -->

    <owl:NamedIndividual rdf:about="http://purl.obolibrary.org/obo/GAZ_00058759">
        <obo:RO_0001025 rdf:resource="http://purl.obolibrary.org/obo/GAZ_00010256"/>
        <obo:IAO_0000115>A lakein northeastern Hawke&apos;s Bay Region, New Zealand.</obo:IAO_0000115>
        <oboInOwl:hasOBONamespace>GAZ</oboInOwl:hasOBONamespace>
        <oboInOwl:id>GAZ:00058759</oboInOwl:id>
        <rdfs:label>Lake Tutira</rdfs:label>
    </owl:NamedIndividual>
    


    <!-- http://purl.obolibrary.org/obo/GAZ_00058760 -->

    <owl:NamedIndividual rdf:about="http://purl.obolibrary.org/obo/GAZ_00058760">
        <obo:RO_0001025 rdf:resource="http://purl.obolibrary.org/obo/GAZ_00009776"/>
        <obo:IAO_0000115>A lake in the city of Wanganui in the North Island of New Zealand.</obo:IAO_0000115>
        <oboInOwl:hasOBONamespace>GAZ</oboInOwl:hasOBONamespace>
        <oboInOwl:id>GAZ:00058760</oboInOwl:id>
        <rdfs:label>Lake Virginia</rdfs:label>
    </owl:NamedIndividual>
    


    <!-- http://purl.obolibrary.org/obo/GAZ_00058761 -->

    <owl:NamedIndividual rdf:about="http://purl.obolibrary.org/obo/GAZ_00058761">
        <obo:RO_0001025 rdf:resource="http://purl.obolibrary.org/obo/GAZ_00004765"/>
        <obo:IAO_0000115>A shallow lake in the upper floodplain of the Waikato River in New Zealand&apos;s North Island. It is a riverine lake, located to the east of Te Kauwhata, 40 km north of Hamilton.</obo:IAO_0000115>
        <oboInOwl:hasOBONamespace>GAZ</oboInOwl:hasOBONamespace>
        <oboInOwl:id>GAZ:00058761</oboInOwl:id>
        <rdfs:label>Lake Waikare</rdfs:label>
    </owl:NamedIndividual>
    


    <!-- http://purl.obolibrary.org/obo/GAZ_00058762 -->

    <owl:NamedIndividual rdf:about="http://purl.obolibrary.org/obo/GAZ_00058762">
        <obo:RO_0001025 rdf:resource="http://purl.obolibrary.org/obo/GAZ_00010256"/>
        <obo:IAO_0000115>A national park located in the north east of the Hawke&apos;s Bay region of the North Island. Established 1954-07-28.</obo:IAO_0000115>
        <oboInOwl:hasOBONamespace>GAZ</oboInOwl:hasOBONamespace>
        <oboInOwl:id>GAZ:00058762</oboInOwl:id>
        <rdfs:label>Te Urewera National Park</rdfs:label>
    </owl:NamedIndividual>
    


    <!-- http://purl.obolibrary.org/obo/GAZ_00058763 -->

    <owl:NamedIndividual rdf:about="http://purl.obolibrary.org/obo/GAZ_00058763">
        <obo:RO_0001025 rdf:resource="http://purl.obolibrary.org/obo/GAZ_00058762"/>
        <obo:IAO_0000115>A lake located in Te Urewera National Park in the North Island of New Zealand, 60 km northwest of Wairoa and 80 km southwest of Gisborne.</obo:IAO_0000115>
        <oboInOwl:hasOBONamespace>GAZ</oboInOwl:hasOBONamespace>
        <oboInOwl:id>GAZ:00058763</oboInOwl:id>
        <rdfs:label>Lake Waikaremoana</rdfs:label>
    </owl:NamedIndividual>
    


    <!-- http://purl.obolibrary.org/obo/GAZ_00058764 -->

    <owl:NamedIndividual rdf:about="http://purl.obolibrary.org/obo/GAZ_00058764">
        <obo:RO_0001025 rdf:resource="http://purl.obolibrary.org/obo/GAZ_00058765"/>
        <obo:IAO_0000115>An island in Lake Waikareiti.</obo:IAO_0000115>
        <oboInOwl:hasOBONamespace>GAZ</oboInOwl:hasOBONamespace>
        <oboInOwl:id>GAZ:00058764</oboInOwl:id>
        <rdfs:label>Rahui Island</rdfs:label>
    </owl:NamedIndividual>
    


    <!-- http://purl.obolibrary.org/obo/GAZ_00058765 -->

    <owl:NamedIndividual rdf:about="http://purl.obolibrary.org/obo/GAZ_00058765">
        <obo:RO_0001025 rdf:resource="http://purl.obolibrary.org/obo/GAZ_00058762"/>
        <obo:IAO_0000115>A lake located in Te Urewera National Park in the North Island of New Zealand. Its formation followed a landslide 18,000 years ago, in which a part of the landmass of 10 km wide slid to the north-west. It is four km to the northeast of the larger Lake Waikaremoana, into which it drains via the Aniwaniwa Stream.</obo:IAO_0000115>
        <oboInOwl:hasOBONamespace>GAZ</oboInOwl:hasOBONamespace>
        <oboInOwl:id>GAZ:00058765</oboInOwl:id>
        <rdfs:label>Lake Waikareiti</rdfs:label>
    </owl:NamedIndividual>
    


    <!-- http://purl.obolibrary.org/obo/GAZ_00058766 -->

    <owl:NamedIndividual rdf:about="http://purl.obolibrary.org/obo/GAZ_00058766">
        <obo:RO_0001025 rdf:resource="http://purl.obolibrary.org/obo/GAZ_00008562"/>
        <obo:IAO_0000115>A shallow freshwater lake in the southern Canterbury region of New Zealand&apos;s South Island. A number of rivers flow into the lagoon, including the Hook River from the north and the Waihao River from the south.</obo:IAO_0000115>
        <oboInOwl:hasOBONamespace>GAZ</oboInOwl:hasOBONamespace>
        <oboInOwl:id>GAZ:00058766</oboInOwl:id>
        <rdfs:label>Wainono Lagoon</rdfs:label>
    </owl:NamedIndividual>
    


    <!-- http://purl.obolibrary.org/obo/GAZ_00058767 -->

    <owl:NamedIndividual rdf:about="http://purl.obolibrary.org/obo/GAZ_00058767">
        <obo:RO_0001025 rdf:resource="http://purl.obolibrary.org/obo/GAZ_00004765"/>
        <obo:IAO_0000115>A lake at the southern end of the North Island of New Zealand, 50 km east of Wellington. The lake&apos;s catchment area is large, and includes the eastern slopes of the Rimutaka and Tararua Ranges. The lake takes water from several rivers and was originally the main outflow for the Ruamahanga. This in turn drained slowly into Palliser Bay and Cook Strait ten km south, via what is now Lake Onoke. The river, however, was diverted in the 1960&apos;s to assist flow, thereby reducing flooding for farmers. The lake today therefore covers an area significantly smaller than its historical size of around 210 km2.</obo:IAO_0000115>
        <oboInOwl:hasOBONamespace>GAZ</oboInOwl:hasOBONamespace>
        <oboInOwl:id>GAZ:00058767</oboInOwl:id>
        <rdfs:label>Lake Wairarapa</rdfs:label>
    </owl:NamedIndividual>
    


    <!-- http://purl.obolibrary.org/obo/GAZ_00058768 -->

    <owl:NamedIndividual rdf:about="http://purl.obolibrary.org/obo/GAZ_00058768">
        <obo:RO_0001025 rdf:resource="http://purl.obolibrary.org/obo/GAZ_00004765"/>
        <obo:IAO_0000115>A reservoir in New Zealand. Waitakere Dam was completed in 1910.</obo:IAO_0000115>
        <oboInOwl:hasOBONamespace>GAZ</oboInOwl:hasOBONamespace>
        <oboInOwl:id>GAZ:00058768</oboInOwl:id>
        <rdfs:label>Waitakere Reservoir</rdfs:label>
    </owl:NamedIndividual>
    


    <!-- http://purl.obolibrary.org/obo/GAZ_00058769 -->

    <owl:NamedIndividual rdf:about="http://purl.obolibrary.org/obo/GAZ_00058769">
        <obo:RO_0001025 rdf:resource="http://purl.obolibrary.org/obo/GAZ_00004764"/>
        <obo:IAO_0000115>A bog lake near Tautuku Bay in the Catlins, south of Dunedin, New Zealand. It formed behind sand dunes after the last ice age, and has gradually shrunk to its current size of 1.7 ha.</obo:IAO_0000115>
        <oboInOwl:hasOBONamespace>GAZ</oboInOwl:hasOBONamespace>
        <oboInOwl:id>GAZ:00058769</oboInOwl:id>
        <rdfs:label>Lake Wilkie</rdfs:label>
    </owl:NamedIndividual>
    


    <!-- http://purl.obolibrary.org/obo/GAZ_00058770 -->

    <owl:NamedIndividual rdf:about="http://purl.obolibrary.org/obo/GAZ_00058770">
        <obo:RO_0001025 rdf:resource="http://purl.obolibrary.org/obo/GAZ_00008562"/>
        <obo:IAO_0000115>A brackish shallow coastal lagoon approximately 1 km N of Timaru, in south Canterbury, New Zealand.</obo:IAO_0000115>
        <oboInOwl:hasOBONamespace>GAZ</oboInOwl:hasOBONamespace>
        <oboInOwl:id>GAZ:00058770</oboInOwl:id>
        <rdfs:label>Washdyke Lagoon</rdfs:label>
    </owl:NamedIndividual>
    


    <!-- http://purl.obolibrary.org/obo/GAZ_00058771 -->

    <owl:NamedIndividual rdf:about="http://purl.obolibrary.org/obo/GAZ_00058771">
        <obo:RO_0001025 rdf:resource="http://purl.obolibrary.org/obo/GAZ_00008562"/>
        <obo:IAO_0000115>A protected area.</obo:IAO_0000115>
        <oboInOwl:hasOBONamespace>GAZ</oboInOwl:hasOBONamespace>
        <oboInOwl:id>GAZ:00058771</oboInOwl:id>
        <rdfs:label>Washdyke Lagoon Wildlife Refuge</rdfs:label>
    </owl:NamedIndividual>
    


    <!-- http://purl.obolibrary.org/obo/GAZ_00087701 -->

    <owl:NamedIndividual rdf:about="http://purl.obolibrary.org/obo/GAZ_00087701">
        <rdf:type rdf:resource="http://purl.obolibrary.org/obo/ENVO_00000167"/>
        <obo:RO_0001025 rdf:resource="http://purl.obolibrary.org/obo/GAZ_00004767"/>
        <obo:IAO_0000115>An estuary in coastal Otago, about 25km north of Dunedin. The Waitati River and Careys Creek enter Blueskin Bay at its southwest and northwest corners. A long sand spit from the northern headland closes the bay to a small channel to the Pacific Ocean at the southeast corner. Rabbit Island lies just inside this entrance.</obo:IAO_0000115>
        <oboInOwl:hasOBONamespace>GAZ</oboInOwl:hasOBONamespace>
        <oboInOwl:id>GAZ:00087701</oboInOwl:id>
        <rdfs:label>Blueskin Bay</rdfs:label>
    </owl:NamedIndividual>
    


    <!-- http://purl.obolibrary.org/obo/GAZ_00087702 -->

    <owl:NamedIndividual rdf:about="http://purl.obolibrary.org/obo/GAZ_00087702">
        <obo:RO_0001025 rdf:resource="http://purl.obolibrary.org/obo/GAZ_00087701"/>
        <obo:IAO_0000115>An island in Blueskin Bay.</obo:IAO_0000115>
        <oboInOwl:hasOBONamespace>GAZ</oboInOwl:hasOBONamespace>
        <oboInOwl:id>GAZ:00087702</oboInOwl:id>
        <rdfs:label>Rabbit Island</rdfs:label>
    </owl:NamedIndividual>
    


    <!-- http://purl.obolibrary.org/obo/GAZ_00087703 -->

    <owl:NamedIndividual rdf:about="http://purl.obolibrary.org/obo/GAZ_00087703">
        <obo:RO_0001025 rdf:resource="http://purl.obolibrary.org/obo/GAZ_00007176"/>
        <obo:IAO_0000115>A reef 10 km to the S of The Snares.</obo:IAO_0000115>
        <oboInOwl:hasOBONamespace>GAZ</oboInOwl:hasOBONamespace>
        <oboInOwl:id>GAZ:00087703</oboInOwl:id>
        <rdfs:label>Seal Reef</rdfs:label>
    </owl:NamedIndividual>
    


    <!-- http://purl.obolibrary.org/obo/GAZ_00088595 -->

    <owl:NamedIndividual rdf:about="http://purl.obolibrary.org/obo/GAZ_00088595">
        <obo:RO_0001025 rdf:resource="http://purl.obolibrary.org/obo/GAZ_00009775"/>
        <obo:IAO_0000115>A national park located in the North Island of New Zealand. It covers an area of 742 km2 bordering the Whanganui River. It incorporates areas of Crown land, former state forest and a number of former reserves. The river itself is not part of the park. The park was established in 1986.</obo:IAO_0000115>
        <oboInOwl:hasOBONamespace>GAZ</oboInOwl:hasOBONamespace>
        <oboInOwl:id>GAZ:00088595</oboInOwl:id>
        <rdfs:label>Whanganui National Park</rdfs:label>
    </owl:NamedIndividual>
    


    <!-- http://purl.obolibrary.org/obo/GAZ_00088596 -->

    <owl:NamedIndividual rdf:about="http://purl.obolibrary.org/obo/GAZ_00088596">
        <obo:RO_0001025 rdf:resource="http://purl.obolibrary.org/obo/GAZ_00004777"/>
        <obo:IAO_0000115>A national park on the west coast of the South Island of New Zealand. Established 1987. The park ranges from on or near the coastline to the peak of the Paparoa Ranges. A separate section of the park is to the north and is centered at Ananui Creek.</obo:IAO_0000115>
        <oboInOwl:hasOBONamespace>GAZ</oboInOwl:hasOBONamespace>
        <oboInOwl:id>GAZ:00088596</oboInOwl:id>
        <rdfs:label>Paparoa National Park</rdfs:label>
    </owl:NamedIndividual>
    


    <!-- http://purl.obolibrary.org/obo/GAZ_00088597 -->

    <owl:NamedIndividual rdf:about="http://purl.obolibrary.org/obo/GAZ_00088597">
        <obo:RO_0001025 rdf:resource="http://purl.obolibrary.org/obo/GAZ_00008562"/>
        <obo:IAO_0000115>A national park located in the South Island of New Zealand. Established 1929.</obo:IAO_0000115>
        <oboInOwl:hasOBONamespace>GAZ</oboInOwl:hasOBONamespace>
        <oboInOwl:id>GAZ:00088597</oboInOwl:id>
        <rdfs:label>Arthur&apos;s Pass National Park</rdfs:label>
    </owl:NamedIndividual>
    


    <!-- http://purl.obolibrary.org/obo/GAZ_00088598 -->

    <owl:NamedIndividual rdf:about="http://purl.obolibrary.org/obo/GAZ_00088598">
        <obo:RO_0001025 rdf:resource="http://purl.obolibrary.org/obo/GAZ_00004777"/>
        <obo:IAO_0000115>A national park located in New Zealand&apos;s South Island. Established in 1960.</obo:IAO_0000115>
        <oboInOwl:hasOBONamespace>GAZ</oboInOwl:hasOBONamespace>
        <oboInOwl:id>GAZ:00088598</oboInOwl:id>
        <rdfs:label>Westland National Park</rdfs:label>
    </owl:NamedIndividual>
    


    <!-- http://purl.obolibrary.org/obo/GAZ_00139394 -->

    <owl:NamedIndividual rdf:about="http://purl.obolibrary.org/obo/GAZ_00139394">
        <obo:RO_0001025 rdf:resource="http://purl.obolibrary.org/obo/GAZ_00017440"/>
        <obo:IAO_0000115>A former (1941-1995) New Zealand research station at the head of Perseverance Bay.</obo:IAO_0000115>
        <oboInOwl:hasOBONamespace>GAZ</oboInOwl:hasOBONamespace>
        <oboInOwl:id>GAZ:00139394</oboInOwl:id>
        <rdfs:label>Campbell Island Station</rdfs:label>
    </owl:NamedIndividual>
    


    <!-- http://purl.obolibrary.org/obo/GAZ_00139395 -->

    <owl:NamedIndividual rdf:about="http://purl.obolibrary.org/obo/GAZ_00139395">
        <obo:RO_0001025 rdf:resource="http://purl.obolibrary.org/obo/GAZ_00007175"/>
        <obo:IAO_0000115>A rock to the NE of Campbell Island, off North Cape.</obo:IAO_0000115>
        <oboInOwl:hasOBONamespace>GAZ</oboInOwl:hasOBONamespace>
        <oboInOwl:id>GAZ:00139395</oboInOwl:id>
        <rdfs:label>Bull Rock</rdfs:label>
    </owl:NamedIndividual>
    


    <!-- http://purl.obolibrary.org/obo/GAZ_00141829 -->

    <owl:NamedIndividual rdf:about="http://purl.obolibrary.org/obo/GAZ_00141829">
        <obo:RO_0001025 rdf:resource="http://purl.obolibrary.org/obo/GAZ_00017417"/>
        <obo:IAO_0000115>A 705 m peak on Adams Island, the second-largest of New Zealand&apos;s Auckland Island chain. It is the highest point in the Auckland Islands. Mount Dick is part of the rim of an extinct volcano, the crater of which now forms Carnley Harbour, which separates Adams Island from the larger Auckland Island.</obo:IAO_0000115>
        <oboInOwl:hasOBONamespace>GAZ</oboInOwl:hasOBONamespace>
        <oboInOwl:id>GAZ:00141829</oboInOwl:id>
        <rdfs:label>Mount Dick</rdfs:label>
    </owl:NamedIndividual>
    


    <!-- http://purl.obolibrary.org/obo/GAZ_00141832 -->

    <owl:NamedIndividual rdf:about="http://purl.obolibrary.org/obo/GAZ_00141832">
        <obo:RO_0001025 rdf:resource="http://purl.obolibrary.org/obo/GAZ_00007175"/>
        <obo:IAO_0000115>One of the Campbell Islands, NW of Courrejolles Point.</obo:IAO_0000115>
        <oboInOwl:hasOBONamespace>GAZ</oboInOwl:hasOBONamespace>
        <oboInOwl:id>GAZ:00141832</oboInOwl:id>
        <rdfs:label>Isle de Jeanette Marie</rdfs:label>
    </owl:NamedIndividual>
    


    <!-- http://purl.obolibrary.org/obo/GAZ_00141833 -->

    <owl:NamedIndividual rdf:about="http://purl.obolibrary.org/obo/GAZ_00141833">
        <obo:RO_0001025 rdf:resource="http://purl.obolibrary.org/obo/GAZ_00007175"/>
        <obo:IAO_0000115>One of the Campbell Islands.</obo:IAO_0000115>
        <oboInOwl:hasOBONamespace>GAZ</oboInOwl:hasOBONamespace>
        <oboInOwl:id>GAZ:00141833</oboInOwl:id>
        <rdfs:label>Monowai Island</rdfs:label>
    </owl:NamedIndividual>
    


    <!-- http://purl.obolibrary.org/obo/GAZ_00141835 -->

    <owl:NamedIndividual rdf:about="http://purl.obolibrary.org/obo/GAZ_00141835">
        <rdf:type rdf:resource="http://purl.obolibrary.org/obo/ENVO_00000305"/>
        <obo:RO_0001025 rdf:resource="http://purl.obolibrary.org/obo/GAZ_00017440"/>
        <obo:IAO_0000115>A headland on the NW of Campbell Island at the end of a NW facing peninsula.</obo:IAO_0000115>
        <oboInOwl:hasOBONamespace>GAZ</oboInOwl:hasOBONamespace>
        <oboInOwl:id>GAZ:00141835</oboInOwl:id>
        <rdfs:label>Courrejolles Point</rdfs:label>
    </owl:NamedIndividual>
    


    <!-- http://purl.obolibrary.org/obo/GAZ_00141836 -->

    <owl:NamedIndividual rdf:about="http://purl.obolibrary.org/obo/GAZ_00141836">
        <obo:RO_0001025 rdf:resource="http://purl.obolibrary.org/obo/GAZ_00017440"/>
        <obo:IAO_0000115>The point marking the S entrance to Perseverance Harbour.</obo:IAO_0000115>
        <oboInOwl:hasOBONamespace>GAZ</oboInOwl:hasOBONamespace>
        <oboInOwl:id>GAZ:00141836</oboInOwl:id>
        <rdfs:label>South Point</rdfs:label>
    </owl:NamedIndividual>
    


    <!-- http://purl.obolibrary.org/obo/GAZ_00141837 -->

    <owl:NamedIndividual rdf:about="http://purl.obolibrary.org/obo/GAZ_00141837">
        <obo:RO_0001025 rdf:resource="http://purl.obolibrary.org/obo/GAZ_00017440"/>
        <obo:IAO_0000115>The point marking the N entrance to Perseverance Harbour.</obo:IAO_0000115>
        <oboInOwl:hasOBONamespace>GAZ</oboInOwl:hasOBONamespace>
        <oboInOwl:id>GAZ:00141837</oboInOwl:id>
        <rdfs:label>Erebus Point</rdfs:label>
    </owl:NamedIndividual>
    


    <!-- http://purl.obolibrary.org/obo/GAZ_00141864 -->

    <owl:NamedIndividual rdf:about="http://purl.obolibrary.org/obo/GAZ_00141864">
        <rdf:type rdf:resource="http://purl.obolibrary.org/obo/ENVO_00000305"/>
        <obo:RO_0001025 rdf:resource="http://purl.obolibrary.org/obo/GAZ_00044991"/>
        <obo:IAO_0000115>A headland of North East Island.</obo:IAO_0000115>
        <oboInOwl:hasOBONamespace>GAZ</oboInOwl:hasOBONamespace>
        <oboInOwl:id>GAZ:00141864</oboInOwl:id>
        <rdfs:label>South Promontory</rdfs:label>
    </owl:NamedIndividual>
    


    <!-- http://purl.obolibrary.org/obo/GAZ_00141865 -->

    <owl:NamedIndividual rdf:about="http://purl.obolibrary.org/obo/GAZ_00141865">
        <obo:RO_0001025 rdf:resource="http://purl.obolibrary.org/obo/GAZ_00007176"/>
        <obo:IAO_0000115>Rocks off the North Promontory of North East Island.</obo:IAO_0000115>
        <oboInOwl:hasOBONamespace>GAZ</oboInOwl:hasOBONamespace>
        <oboInOwl:id>GAZ:00141865</oboInOwl:id>
        <rdfs:label>North Daption</rdfs:label>
    </owl:NamedIndividual>
    


    <!-- http://purl.obolibrary.org/obo/GAZ_00141866 -->

    <owl:NamedIndividual rdf:about="http://purl.obolibrary.org/obo/GAZ_00141866">
        <obo:RO_0001025 rdf:resource="http://purl.obolibrary.org/obo/GAZ_00007176"/>
        <obo:IAO_0000115>Rocks off the North Promontory of North East Island.</obo:IAO_0000115>
        <oboInOwl:hasOBONamespace>GAZ</oboInOwl:hasOBONamespace>
        <oboInOwl:id>GAZ:00141866</oboInOwl:id>
        <rdfs:label>South Daption</rdfs:label>
    </owl:NamedIndividual>
    


    <!-- http://purl.obolibrary.org/obo/GAZ_00141867 -->

    <owl:NamedIndividual rdf:about="http://purl.obolibrary.org/obo/GAZ_00141867">
        <obo:RO_0001025 rdf:resource="http://purl.obolibrary.org/obo/GAZ_00007176"/>
        <obo:IAO_0000115>A small island S of the W peninsula of North East Island.</obo:IAO_0000115>
        <oboInOwl:hasOBONamespace>GAZ</oboInOwl:hasOBONamespace>
        <oboInOwl:id>GAZ:00141867</oboInOwl:id>
        <rdfs:label>Alert Stack</rdfs:label>
    </owl:NamedIndividual>
    


    <!-- http://purl.obolibrary.org/obo/GAZ_00141868 -->

    <owl:NamedIndividual rdf:about="http://purl.obolibrary.org/obo/GAZ_00141868">
        <rdf:type rdf:resource="http://purl.obolibrary.org/obo/ENVO_00000305"/>
        <obo:RO_0001025 rdf:resource="http://purl.obolibrary.org/obo/GAZ_00044991"/>
        <obo:IAO_0000115>A headland of North East Island.</obo:IAO_0000115>
        <oboInOwl:hasOBONamespace>GAZ</oboInOwl:hasOBONamespace>
        <oboInOwl:id>GAZ:00141868</oboInOwl:id>
        <rdfs:label>North Promontory</rdfs:label>
    </owl:NamedIndividual>
    


    <!-- http://purl.obolibrary.org/obo/GAZ_00141977 -->

    <owl:NamedIndividual rdf:about="http://purl.obolibrary.org/obo/GAZ_00141977">
        <obo:RO_0001025 rdf:resource="http://purl.obolibrary.org/obo/GAZ_00007172"/>
        <obo:IAO_0000115>An island off the E coast of Antipodes Island.</obo:IAO_0000115>
        <oboInOwl:hasOBONamespace>GAZ</oboInOwl:hasOBONamespace>
        <oboInOwl:id>GAZ:00141977</oboInOwl:id>
        <rdfs:label>Leeward Island</rdfs:label>
    </owl:NamedIndividual>
    


    <!-- http://purl.obolibrary.org/obo/GAZ_00141978 -->

    <owl:NamedIndividual rdf:about="http://purl.obolibrary.org/obo/GAZ_00141978">
        <obo:RO_0001025 rdf:resource="http://purl.obolibrary.org/obo/GAZ_00007172"/>
        <obo:IAO_0000115>A small island off the N coast of Antipodes Island.</obo:IAO_0000115>
        <oboInOwl:hasOBONamespace>GAZ</oboInOwl:hasOBONamespace>
        <oboInOwl:id>GAZ:00141978</oboInOwl:id>
        <rdfs:label>Orde Lees Islet</rdfs:label>
    </owl:NamedIndividual>
    


    <!-- http://purl.obolibrary.org/obo/GAZ_00141979 -->

    <owl:NamedIndividual rdf:about="http://purl.obolibrary.org/obo/GAZ_00141979">
        <obo:RO_0001025 rdf:resource="http://purl.obolibrary.org/obo/GAZ_00007172"/>
        <obo:IAO_0000115>Two islands off the NW coast of Antipodes Island.</obo:IAO_0000115>
        <oboInOwl:hasOBONamespace>GAZ</oboInOwl:hasOBONamespace>
        <oboInOwl:id>GAZ:00141979</oboInOwl:id>
        <rdfs:label>Winward Islands</rdfs:label>
    </owl:NamedIndividual>
    


    <!-- http://purl.obolibrary.org/obo/GAZ_00141980 -->

    <owl:NamedIndividual rdf:about="http://purl.obolibrary.org/obo/GAZ_00141980">
        <obo:RO_0001025 rdf:resource="http://purl.obolibrary.org/obo/GAZ_00044917"/>
        <obo:IAO_0000115>The most westerly point of Antipodes Island.</obo:IAO_0000115>
        <oboInOwl:hasOBONamespace>GAZ</oboInOwl:hasOBONamespace>
        <oboInOwl:id>GAZ:00141980</oboInOwl:id>
        <rdfs:label>Cave Point</rdfs:label>
    </owl:NamedIndividual>
    


    <!-- http://purl.obolibrary.org/obo/GAZ_00141981 -->

    <owl:NamedIndividual rdf:about="http://purl.obolibrary.org/obo/GAZ_00141981">
        <obo:RO_0001025 rdf:resource="http://purl.obolibrary.org/obo/GAZ_00044917"/>
        <obo:IAO_0000115>The N peninusula of Antipodes Island.</obo:IAO_0000115>
        <oboInOwl:hasOBONamespace>GAZ</oboInOwl:hasOBONamespace>
        <oboInOwl:id>GAZ:00141981</oboInOwl:id>
        <rdfs:label>Perpendicular Head</rdfs:label>
    </owl:NamedIndividual>
    


    <!-- http://purl.obolibrary.org/obo/GAZ_00141982 -->

    <owl:NamedIndividual rdf:about="http://purl.obolibrary.org/obo/GAZ_00141982">
        <rdf:type rdf:resource="http://purl.obolibrary.org/obo/ENVO_00000167"/>
        <obo:RO_0001025 rdf:resource="http://purl.obolibrary.org/obo/GAZ_00044917"/>
        <obo:IAO_0000115>A NE point on Antipodes Island.</obo:IAO_0000115>
        <oboInOwl:hasOBONamespace>GAZ</oboInOwl:hasOBONamespace>
        <oboInOwl:id>GAZ:00141982</oboInOwl:id>
        <rdfs:label>Reef Point</rdfs:label>
    </owl:NamedIndividual>
    


    <!-- http://purl.obolibrary.org/obo/GAZ_00141983 -->

    <owl:NamedIndividual rdf:about="http://purl.obolibrary.org/obo/GAZ_00141983">
        <rdf:type rdf:resource="http://purl.obolibrary.org/obo/ENVO_00000167"/>
        <obo:RO_0001025 rdf:resource="http://purl.obolibrary.org/obo/GAZ_00044917"/>
        <obo:IAO_0000115>A SE point of Antipodes Island.</obo:IAO_0000115>
        <oboInOwl:hasOBONamespace>GAZ</oboInOwl:hasOBONamespace>
        <oboInOwl:id>GAZ:00141983</oboInOwl:id>
        <rdfs:label>Albatross Head</rdfs:label>
    </owl:NamedIndividual>
    


    <!-- http://purl.obolibrary.org/obo/GAZ_00141984 -->

    <owl:NamedIndividual rdf:about="http://purl.obolibrary.org/obo/GAZ_00141984">
        <obo:RO_0001025 rdf:resource="http://purl.obolibrary.org/obo/GAZ_00141981"/>
        <obo:IAO_0000115>The most northerly point of Antipodes Island.</obo:IAO_0000115>
        <oboInOwl:hasOBONamespace>GAZ</oboInOwl:hasOBONamespace>
        <oboInOwl:id>GAZ:00141984</oboInOwl:id>
        <rdfs:label>North Cape</rdfs:label>
    </owl:NamedIndividual>
    


    <!-- http://purl.obolibrary.org/obo/GAZ_00142011 -->

    <owl:NamedIndividual rdf:about="http://purl.obolibrary.org/obo/GAZ_00142011">
        <obo:RO_0001025 rdf:resource="http://purl.obolibrary.org/obo/GAZ_00044989"/>
        <obo:IAO_0000115>A rock NE of the Western Chain Islands.</obo:IAO_0000115>
        <oboInOwl:hasOBONamespace>GAZ</oboInOwl:hasOBONamespace>
        <oboInOwl:id>GAZ:00142011</oboInOwl:id>
        <rdfs:label>Vancouver Rock</rdfs:label>
    </owl:NamedIndividual>
    


    <!-- http://purl.obolibrary.org/obo/GAZ_00142019 -->

    <owl:NamedIndividual rdf:about="http://purl.obolibrary.org/obo/GAZ_00142019">
        <rdf:type rdf:resource="http://purl.obolibrary.org/obo/ENVO_00000305"/>
        <obo:RO_0001025 rdf:resource="http://purl.obolibrary.org/obo/GAZ_00044991"/>
        <obo:IAO_0000115>A headland on the E coast of North East Island, S of Seal Point.</obo:IAO_0000115>
        <oboInOwl:hasOBONamespace>GAZ</oboInOwl:hasOBONamespace>
        <oboInOwl:id>GAZ:00142019</oboInOwl:id>
        <rdfs:label>Station Point</rdfs:label>
    </owl:NamedIndividual>
    


    <!-- http://purl.obolibrary.org/obo/GAZ_00142022 -->

    <owl:NamedIndividual rdf:about="http://purl.obolibrary.org/obo/GAZ_00142022">
        <obo:RO_0001025 rdf:resource="http://purl.obolibrary.org/obo/GAZ_00006949"/>
        <obo:IAO_0000115>A group of 42 coral islets within Tokelau in the south Pacific Ocean. Sits atop the Atafu Seamount.</obo:IAO_0000115>
        <oboInOwl:hasOBONamespace>GAZ</oboInOwl:hasOBONamespace>
        <oboInOwl:id>GAZ:00142022</oboInOwl:id>
        <rdfs:label>Atafu Atoll</rdfs:label>
    </owl:NamedIndividual>
    


    <!-- http://purl.obolibrary.org/obo/GAZ_00142024 -->

    <owl:NamedIndividual rdf:about="http://purl.obolibrary.org/obo/GAZ_00142024">
        <obo:RO_0001025 rdf:resource="http://purl.obolibrary.org/obo/GAZ_00142028"/>
        <obo:IAO_0000115>The most N region of the Unamed Island, SE of Tuagatulu.</obo:IAO_0000115>
        <oboInOwl:hasOBONamespace>GAZ</oboInOwl:hasOBONamespace>
        <oboInOwl:id>GAZ:00142024</oboInOwl:id>
        <rdfs:label>Laualalava</rdfs:label>
    </owl:NamedIndividual>
    


    <!-- http://purl.obolibrary.org/obo/GAZ_00142025 -->

    <owl:NamedIndividual rdf:about="http://purl.obolibrary.org/obo/GAZ_00142025">
        <obo:RO_0001025 rdf:resource="http://purl.obolibrary.org/obo/GAZ_00009562"/>
        <obo:IAO_0000115>The NW reef of the Atufa Atoll.</obo:IAO_0000115>
        <oboInOwl:hasOBONamespace>GAZ</oboInOwl:hasOBONamespace>
        <oboInOwl:id>GAZ:00142025</oboInOwl:id>
        <rdfs:label>Ahaga Loa</rdfs:label>
    </owl:NamedIndividual>
    


    <!-- http://purl.obolibrary.org/obo/GAZ_00142027 -->

    <owl:NamedIndividual rdf:about="http://purl.obolibrary.org/obo/GAZ_00142027">
        <obo:RO_0001025 rdf:resource="http://purl.obolibrary.org/obo/GAZ_00009562"/>
        <obo:IAO_0000115>The SE reef of Atafu Atoll.</obo:IAO_0000115>
        <oboInOwl:hasOBONamespace>GAZ</oboInOwl:hasOBONamespace>
        <oboInOwl:id>GAZ:00142027</oboInOwl:id>
        <rdfs:label>Telafu</rdfs:label>
    </owl:NamedIndividual>
    


    <!-- http://purl.obolibrary.org/obo/GAZ_00142028 -->

    <owl:NamedIndividual rdf:about="http://purl.obolibrary.org/obo/GAZ_00142028">
        <obo:RO_0001025 rdf:resource="http://purl.obolibrary.org/obo/GAZ_00142027"/>
        <obo:IAO_0000115>An complex island, apparently not named, at the SE corner of the Atafu Atoll.</obo:IAO_0000115>
        <oboInOwl:hasOBONamespace>GAZ</oboInOwl:hasOBONamespace>
        <oboInOwl:id>GAZ:00142028</oboInOwl:id>
        <rdfs:label>Unnamed Island</rdfs:label>
    </owl:NamedIndividual>
    


    <!-- http://purl.obolibrary.org/obo/GAZ_00142029 -->

    <owl:NamedIndividual rdf:about="http://purl.obolibrary.org/obo/GAZ_00142029">
        <obo:RO_0001025 rdf:resource="http://purl.obolibrary.org/obo/GAZ_00009562"/>
        <obo:IAO_0000115>The NE and E reef of the Atafu Atoll.</obo:IAO_0000115>
        <oboInOwl:hasOBONamespace>GAZ</oboInOwl:hasOBONamespace>
        <oboInOwl:id>GAZ:00142029</oboInOwl:id>
        <rdfs:label>Motu Haka</rdfs:label>
    </owl:NamedIndividual>
    


    <!-- http://purl.obolibrary.org/obo/GAZ_00142030 -->

    <owl:NamedIndividual rdf:about="http://purl.obolibrary.org/obo/GAZ_00142030">
        <obo:RO_0001025 rdf:resource="http://purl.obolibrary.org/obo/GAZ_00009562"/>
        <obo:IAO_0000115>The S reef of the Atafu Atoll.</obo:IAO_0000115>
        <oboInOwl:hasOBONamespace>GAZ</oboInOwl:hasOBONamespace>
        <oboInOwl:id>GAZ:00142030</oboInOwl:id>
        <rdfs:label>Te Atu Hakea</rdfs:label>
    </owl:NamedIndividual>
    


    <!-- http://purl.obolibrary.org/obo/GAZ_00142031 -->

    <owl:NamedIndividual rdf:about="http://purl.obolibrary.org/obo/GAZ_00142031">
        <obo:RO_0001025 rdf:resource="http://purl.obolibrary.org/obo/GAZ_00142029"/>
        <obo:IAO_0000115>The most NE of the islands of the Atafu Atoll.</obo:IAO_0000115>
        <oboInOwl:hasOBONamespace>GAZ</oboInOwl:hasOBONamespace>
        <oboInOwl:id>GAZ:00142031</oboInOwl:id>
        <rdfs:label>Ofaga Matuku</rdfs:label>
    </owl:NamedIndividual>
    


    <!-- http://purl.obolibrary.org/obo/GAZ_00142032 -->

    <owl:NamedIndividual rdf:about="http://purl.obolibrary.org/obo/GAZ_00142032">
        <obo:RO_0001025 rdf:resource="http://purl.obolibrary.org/obo/GAZ_00142031"/>
        <obo:IAO_0000115>The W arm of Ofaga Matuku.</obo:IAO_0000115>
        <oboInOwl:hasOBONamespace>GAZ</oboInOwl:hasOBONamespace>
        <oboInOwl:id>GAZ:00142032</oboInOwl:id>
        <rdfs:label>Te Oki</rdfs:label>
    </owl:NamedIndividual>
    


    <!-- http://purl.obolibrary.org/obo/GAZ_00142033 -->

    <owl:NamedIndividual rdf:about="http://purl.obolibrary.org/obo/GAZ_00142033">
        <obo:RO_0001025 rdf:resource="http://purl.obolibrary.org/obo/GAZ_00142031"/>
        <obo:IAO_0000115>The SE arm of Ofaga Matuku.</obo:IAO_0000115>
        <oboInOwl:hasOBONamespace>GAZ</oboInOwl:hasOBONamespace>
        <oboInOwl:id>GAZ:00142033</oboInOwl:id>
        <rdfs:label>Tuagatulu</rdfs:label>
    </owl:NamedIndividual>
    


    <!-- http://purl.obolibrary.org/obo/GAZ_00142034 -->

    <owl:NamedIndividual rdf:about="http://purl.obolibrary.org/obo/GAZ_00142034">
        <obo:RO_0001025 rdf:resource="http://purl.obolibrary.org/obo/GAZ_00142031"/>
        <obo:IAO_0000115>The central and most N region of Ofaga Matuku.</obo:IAO_0000115>
        <oboInOwl:hasOBONamespace>GAZ</oboInOwl:hasOBONamespace>
        <oboInOwl:id>GAZ:00142034</oboInOwl:id>
        <rdfs:label>Kokoloa</rdfs:label>
    </owl:NamedIndividual>
    


    <!-- http://purl.obolibrary.org/obo/GAZ_00142035 -->

    <owl:NamedIndividual rdf:about="http://purl.obolibrary.org/obo/GAZ_00142035">
        <obo:RO_0001025 rdf:resource="http://purl.obolibrary.org/obo/GAZ_00142028"/>
        <obo:IAO_0000115>The most E region of the Unamed Island.</obo:IAO_0000115>
        <oboInOwl:hasOBONamespace>GAZ</oboInOwl:hasOBONamespace>
        <oboInOwl:id>GAZ:00142035</oboInOwl:id>
        <rdfs:label>Na Utua</rdfs:label>
    </owl:NamedIndividual>
    


    <!-- http://purl.obolibrary.org/obo/GAZ_00142036 -->

    <owl:NamedIndividual rdf:about="http://purl.obolibrary.org/obo/GAZ_00142036">
        <obo:RO_0001025 rdf:resource="http://purl.obolibrary.org/obo/GAZ_00142028"/>
        <obo:IAO_0000115>The central region of the Unamed Island.</obo:IAO_0000115>
        <oboInOwl:hasOBONamespace>GAZ</oboInOwl:hasOBONamespace>
        <oboInOwl:id>GAZ:00142036</oboInOwl:id>
        <rdfs:label>Matalia</rdfs:label>
    </owl:NamedIndividual>
    


    <!-- http://purl.obolibrary.org/obo/GAZ_00142037 -->

    <owl:NamedIndividual rdf:about="http://purl.obolibrary.org/obo/GAZ_00142037">
        <obo:RO_0001025 rdf:resource="http://purl.obolibrary.org/obo/GAZ_00142028"/>
        <obo:IAO_0000115>The S region of the Unamed Island.</obo:IAO_0000115>
        <oboInOwl:hasOBONamespace>GAZ</oboInOwl:hasOBONamespace>
        <oboInOwl:id>GAZ:00142037</oboInOwl:id>
        <rdfs:label>Olopuka</rdfs:label>
    </owl:NamedIndividual>
    


    <!-- http://purl.obolibrary.org/obo/GAZ_00142038 -->

    <owl:NamedIndividual rdf:about="http://purl.obolibrary.org/obo/GAZ_00142038">
        <obo:RO_0001025 rdf:resource="http://purl.obolibrary.org/obo/GAZ_00142039"/>
        <obo:IAO_0000115>The SW of the islands of the Atafu Atoll.</obo:IAO_0000115>
        <oboInOwl:hasOBONamespace>GAZ</oboInOwl:hasOBONamespace>
        <oboInOwl:id>GAZ:00142038</oboInOwl:id>
        <rdfs:label>Fenualoa</rdfs:label>
    </owl:NamedIndividual>
    


    <!-- http://purl.obolibrary.org/obo/GAZ_00142039 -->

    <owl:NamedIndividual rdf:about="http://purl.obolibrary.org/obo/GAZ_00142039">
        <obo:RO_0001025 rdf:resource="http://purl.obolibrary.org/obo/GAZ_00009562"/>
        <obo:IAO_0000115>The SW reef of the Atafu Atoll.</obo:IAO_0000115>
        <oboInOwl:hasOBONamespace>GAZ</oboInOwl:hasOBONamespace>
        <oboInOwl:id>GAZ:00142039</oboInOwl:id>
        <rdfs:label>Te Utua O Henua Loa</rdfs:label>
    </owl:NamedIndividual>
    


    <!-- http://purl.obolibrary.org/obo/GAZ_00142040 -->

    <owl:NamedIndividual rdf:about="http://purl.obolibrary.org/obo/GAZ_00142040">
        <obo:RO_0001025 rdf:resource="http://purl.obolibrary.org/obo/GAZ_00142038"/>
        <obo:IAO_0000115>A small island N of Fenualoa.</obo:IAO_0000115>
        <oboInOwl:hasOBONamespace>GAZ</oboInOwl:hasOBONamespace>
        <oboInOwl:id>GAZ:00142040</oboInOwl:id>
        <rdfs:label>Te Tunoa</rdfs:label>
    </owl:NamedIndividual>
    


    <!-- http://purl.obolibrary.org/obo/GAZ_00142041 -->

    <owl:NamedIndividual rdf:about="http://purl.obolibrary.org/obo/GAZ_00142041">
        <obo:RO_0001025 rdf:resource="http://purl.obolibrary.org/obo/GAZ_00142030"/>
        <obo:IAO_0000115>A small island on the S rim of the Atufa Atoll.</obo:IAO_0000115>
        <oboInOwl:hasOBONamespace>GAZ</oboInOwl:hasOBONamespace>
        <oboInOwl:id>GAZ:00142041</oboInOwl:id>
        <rdfs:label>Motu Fakalolo</rdfs:label>
    </owl:NamedIndividual>
    


    <!-- http://purl.obolibrary.org/obo/GAZ_00142042 -->

    <owl:NamedIndividual rdf:about="http://purl.obolibrary.org/obo/GAZ_00142042">
        <obo:RO_0001025 rdf:resource="http://purl.obolibrary.org/obo/GAZ_00142030"/>
        <obo:IAO_0000115>A small island on the S rim of the Atufa Atoll.</obo:IAO_0000115>
        <oboInOwl:hasOBONamespace>GAZ</oboInOwl:hasOBONamespace>
        <oboInOwl:id>GAZ:00142042</oboInOwl:id>
        <rdfs:label>Motu O Te Lakia</rdfs:label>
    </owl:NamedIndividual>
    


    <!-- http://purl.obolibrary.org/obo/GAZ_00142043 -->

    <owl:NamedIndividual rdf:about="http://purl.obolibrary.org/obo/GAZ_00142043">
        <obo:RO_0001025 rdf:resource="http://purl.obolibrary.org/obo/GAZ_00142030"/>
        <obo:IAO_0000115>A small island on the S rim of the Atufa Atoll.</obo:IAO_0000115>
        <oboInOwl:hasOBONamespace>GAZ</oboInOwl:hasOBONamespace>
        <oboInOwl:id>GAZ:00142043</oboInOwl:id>
        <rdfs:label>Motu Atea</rdfs:label>
    </owl:NamedIndividual>
    


    <!-- http://purl.obolibrary.org/obo/GAZ_00142044 -->

    <owl:NamedIndividual rdf:about="http://purl.obolibrary.org/obo/GAZ_00142044">
        <obo:RO_0001025 rdf:resource="http://purl.obolibrary.org/obo/GAZ_00142030"/>
        <obo:IAO_0000115>A small island on the S rim of the Atufa Atoll.</obo:IAO_0000115>
        <oboInOwl:hasOBONamespace>GAZ</oboInOwl:hasOBONamespace>
        <oboInOwl:id>GAZ:00142044</oboInOwl:id>
        <rdfs:label>Tagi a Kuli</rdfs:label>
    </owl:NamedIndividual>
    


    <!-- http://purl.obolibrary.org/obo/GAZ_00142045 -->

    <owl:NamedIndividual rdf:about="http://purl.obolibrary.org/obo/GAZ_00142045">
        <obo:RO_0001025 rdf:resource="http://purl.obolibrary.org/obo/GAZ_00142030"/>
        <obo:IAO_0000115>A small island on the S rim of the Atufa Atoll.</obo:IAO_0000115>
        <oboInOwl:hasOBONamespace>GAZ</oboInOwl:hasOBONamespace>
        <oboInOwl:id>GAZ:00142045</oboInOwl:id>
        <rdfs:label>Tama Hakea</rdfs:label>
    </owl:NamedIndividual>
    


    <!-- http://purl.obolibrary.org/obo/GAZ_00142046 -->

    <owl:NamedIndividual rdf:about="http://purl.obolibrary.org/obo/GAZ_00142046">
        <obo:RO_0001025 rdf:resource="http://purl.obolibrary.org/obo/GAZ_00142030"/>
        <obo:IAO_0000115>A small island on the S rim of the Atufa Atoll.</obo:IAO_0000115>
        <oboInOwl:hasOBONamespace>GAZ</oboInOwl:hasOBONamespace>
        <oboInOwl:id>GAZ:00142046</oboInOwl:id>
        <rdfs:label>Tulua a Kovi</rdfs:label>
    </owl:NamedIndividual>
    


    <!-- http://purl.obolibrary.org/obo/GAZ_00142047 -->

    <owl:NamedIndividual rdf:about="http://purl.obolibrary.org/obo/GAZ_00142047">
        <obo:RO_0001025 rdf:resource="http://purl.obolibrary.org/obo/GAZ_00142030"/>
        <obo:IAO_0000115>A small island on the S rim of the Atufa Atoll.</obo:IAO_0000115>
        <oboInOwl:hasOBONamespace>GAZ</oboInOwl:hasOBONamespace>
        <oboInOwl:id>GAZ:00142047</oboInOwl:id>
        <rdfs:label>Tulua a Kava</rdfs:label>
    </owl:NamedIndividual>
    


    <!-- http://purl.obolibrary.org/obo/GAZ_00142048 -->

    <owl:NamedIndividual rdf:about="http://purl.obolibrary.org/obo/GAZ_00142048">
        <obo:RO_0001025 rdf:resource="http://purl.obolibrary.org/obo/GAZ_00142030"/>
        <obo:IAO_0000115>A small island on the S rim of the Atufa Atoll.</obo:IAO_0000115>
        <oboInOwl:hasOBONamespace>GAZ</oboInOwl:hasOBONamespace>
        <oboInOwl:id>GAZ:00142048</oboInOwl:id>
        <rdfs:label>Hakea Lahi Ki Matagi</rdfs:label>
    </owl:NamedIndividual>
    


    <!-- http://purl.obolibrary.org/obo/GAZ_00142049 -->

    <owl:NamedIndividual rdf:about="http://purl.obolibrary.org/obo/GAZ_00142049">
        <obo:RO_0001025 rdf:resource="http://purl.obolibrary.org/obo/GAZ_00142030"/>
        <obo:IAO_0000115>A small island on the S rim of the Atufa Atoll.</obo:IAO_0000115>
        <oboInOwl:hasOBONamespace>GAZ</oboInOwl:hasOBONamespace>
        <oboInOwl:id>GAZ:00142049</oboInOwl:id>
        <rdfs:label>Motu O Tenumi</rdfs:label>
    </owl:NamedIndividual>
    


    <!-- http://purl.obolibrary.org/obo/GAZ_00142050 -->

    <owl:NamedIndividual rdf:about="http://purl.obolibrary.org/obo/GAZ_00142050">
        <obo:RO_0001025 rdf:resource="http://purl.obolibrary.org/obo/GAZ_00142030"/>
        <obo:IAO_0000115>A small island on the S rim of the Atufa Atoll.</obo:IAO_0000115>
        <oboInOwl:hasOBONamespace>GAZ</oboInOwl:hasOBONamespace>
        <oboInOwl:id>GAZ:00142050</oboInOwl:id>
        <rdfs:label>Malutea</rdfs:label>
    </owl:NamedIndividual>
    


    <!-- http://purl.obolibrary.org/obo/GAZ_00142051 -->

    <owl:NamedIndividual rdf:about="http://purl.obolibrary.org/obo/GAZ_00142051">
        <obo:RO_0001025 rdf:resource="http://purl.obolibrary.org/obo/GAZ_00142030"/>
        <obo:IAO_0000115>A small island on the S rim of the Atufa Atoll.</obo:IAO_0000115>
        <oboInOwl:hasOBONamespace>GAZ</oboInOwl:hasOBONamespace>
        <oboInOwl:id>GAZ:00142051</oboInOwl:id>
        <rdfs:label>Hakea O Himi</rdfs:label>
    </owl:NamedIndividual>
    


    <!-- http://purl.obolibrary.org/obo/GAZ_00142052 -->

    <owl:NamedIndividual rdf:about="http://purl.obolibrary.org/obo/GAZ_00142052">
        <obo:RO_0001025 rdf:resource="http://purl.obolibrary.org/obo/GAZ_00142030"/>
        <obo:IAO_0000115>A small island on the S rim of the Atufa Atoll.</obo:IAO_0000115>
        <oboInOwl:hasOBONamespace>GAZ</oboInOwl:hasOBONamespace>
        <oboInOwl:id>GAZ:00142052</oboInOwl:id>
        <rdfs:label>Hakea o Fata</rdfs:label>
    </owl:NamedIndividual>
    


    <!-- http://purl.obolibrary.org/obo/GAZ_00142053 -->

    <owl:NamedIndividual rdf:about="http://purl.obolibrary.org/obo/GAZ_00142053">
        <obo:RO_0001025 rdf:resource="http://purl.obolibrary.org/obo/GAZ_00142030"/>
        <obo:IAO_0000115>A small island on the S rim of the Atufa Atoll.</obo:IAO_0000115>
        <oboInOwl:hasOBONamespace>GAZ</oboInOwl:hasOBONamespace>
        <oboInOwl:id>GAZ:00142053</oboInOwl:id>
        <rdfs:label>Motu Te Niu</rdfs:label>
    </owl:NamedIndividual>
    


    <!-- http://purl.obolibrary.org/obo/GAZ_00142054 -->

    <owl:NamedIndividual rdf:about="http://purl.obolibrary.org/obo/GAZ_00142054">
        <obo:RO_0001025 rdf:resource="http://purl.obolibrary.org/obo/GAZ_00142030"/>
        <obo:IAO_0000115>A small island on the S rim of the Atufa Atoll.</obo:IAO_0000115>
        <oboInOwl:hasOBONamespace>GAZ</oboInOwl:hasOBONamespace>
        <oboInOwl:id>GAZ:00142054</oboInOwl:id>
        <rdfs:label>Kenakena</rdfs:label>
    </owl:NamedIndividual>
    


    <!-- http://purl.obolibrary.org/obo/GAZ_00142055 -->

    <owl:NamedIndividual rdf:about="http://purl.obolibrary.org/obo/GAZ_00142055">
        <obo:RO_0001025 rdf:resource="http://purl.obolibrary.org/obo/GAZ_00142030"/>
        <obo:IAO_0000115>A small island on the S rim of the Atufa Atoll.</obo:IAO_0000115>
        <oboInOwl:hasOBONamespace>GAZ</oboInOwl:hasOBONamespace>
        <oboInOwl:id>GAZ:00142055</oboInOwl:id>
        <rdfs:label>Hakea O Hoi</rdfs:label>
    </owl:NamedIndividual>
    


    <!-- http://purl.obolibrary.org/obo/GAZ_00142056 -->

    <owl:NamedIndividual rdf:about="http://purl.obolibrary.org/obo/GAZ_00142056">
        <obo:RO_0001025 rdf:resource="http://purl.obolibrary.org/obo/GAZ_00142030"/>
        <obo:IAO_0000115>A small island on the S rim of the Atufa Atoll.</obo:IAO_0000115>
        <oboInOwl:hasOBONamespace>GAZ</oboInOwl:hasOBONamespace>
        <oboInOwl:id>GAZ:00142056</oboInOwl:id>
        <rdfs:label>Motu Fakakaka</rdfs:label>
    </owl:NamedIndividual>
    


    <!-- http://purl.obolibrary.org/obo/GAZ_00142057 -->

    <owl:NamedIndividual rdf:about="http://purl.obolibrary.org/obo/GAZ_00142057">
        <obo:RO_0001025 rdf:resource="http://purl.obolibrary.org/obo/GAZ_00142030"/>
        <obo:IAO_0000115>A small island on the S rim of the Atufa Atoll.</obo:IAO_0000115>
        <oboInOwl:hasOBONamespace>GAZ</oboInOwl:hasOBONamespace>
        <oboInOwl:id>GAZ:00142057</oboInOwl:id>
        <rdfs:label>Hotoma</rdfs:label>
    </owl:NamedIndividual>
    


    <!-- http://purl.obolibrary.org/obo/GAZ_00142058 -->

    <owl:NamedIndividual rdf:about="http://purl.obolibrary.org/obo/GAZ_00142058">
        <obo:RO_0001025 rdf:resource="http://purl.obolibrary.org/obo/GAZ_00142030"/>
        <obo:IAO_0000115>A small island on the S rim of the Atufa Atoll.</obo:IAO_0000115>
        <oboInOwl:hasOBONamespace>GAZ</oboInOwl:hasOBONamespace>
        <oboInOwl:id>GAZ:00142058</oboInOwl:id>
        <rdfs:label>Niuefa</rdfs:label>
    </owl:NamedIndividual>
    


    <!-- http://purl.obolibrary.org/obo/GAZ_00142059 -->

    <owl:NamedIndividual rdf:about="http://purl.obolibrary.org/obo/GAZ_00142059">
        <obo:RO_0001025 rdf:resource="http://purl.obolibrary.org/obo/GAZ_00142030"/>
        <obo:IAO_0000115>A small island on the S rim of the Atufa Atoll.</obo:IAO_0000115>
        <oboInOwl:hasOBONamespace>GAZ</oboInOwl:hasOBONamespace>
        <oboInOwl:id>GAZ:00142059</oboInOwl:id>
        <rdfs:label>Tatega</rdfs:label>
    </owl:NamedIndividual>
    


    <!-- http://purl.obolibrary.org/obo/GAZ_00142060 -->

    <owl:NamedIndividual rdf:about="http://purl.obolibrary.org/obo/GAZ_00142060">
        <obo:RO_0001025 rdf:resource="http://purl.obolibrary.org/obo/GAZ_00142030"/>
        <obo:IAO_0000115>A small island on the S rim of the Atufa Atoll.</obo:IAO_0000115>
        <oboInOwl:hasOBONamespace>GAZ</oboInOwl:hasOBONamespace>
        <oboInOwl:id>GAZ:00142060</oboInOwl:id>
        <rdfs:label>Komulo</rdfs:label>
    </owl:NamedIndividual>
    


    <!-- http://purl.obolibrary.org/obo/GAZ_00142061 -->

    <owl:NamedIndividual rdf:about="http://purl.obolibrary.org/obo/GAZ_00142061">
        <obo:RO_0001025 rdf:resource="http://purl.obolibrary.org/obo/GAZ_00142030"/>
        <obo:IAO_0000115>A small island on the S rim of the Atufa Atoll.</obo:IAO_0000115>
        <oboInOwl:hasOBONamespace>GAZ</oboInOwl:hasOBONamespace>
        <oboInOwl:id>GAZ:00142061</oboInOwl:id>
        <rdfs:label>Moti O Te Fala</rdfs:label>
    </owl:NamedIndividual>
    


    <!-- http://purl.obolibrary.org/obo/GAZ_00142062 -->

    <owl:NamedIndividual rdf:about="http://purl.obolibrary.org/obo/GAZ_00142062">
        <obo:RO_0001025 rdf:resource="http://purl.obolibrary.org/obo/GAZ_00142030"/>
        <obo:IAO_0000115>A small island on the S rim of the Atufa Atoll.</obo:IAO_0000115>
        <oboInOwl:hasOBONamespace>GAZ</oboInOwl:hasOBONamespace>
        <oboInOwl:id>GAZ:00142062</oboInOwl:id>
        <rdfs:label>Malo O Futa</rdfs:label>
    </owl:NamedIndividual>
    


    <!-- http://purl.obolibrary.org/obo/GAZ_00142063 -->

    <owl:NamedIndividual rdf:about="http://purl.obolibrary.org/obo/GAZ_00142063">
        <obo:RO_0001025 rdf:resource="http://purl.obolibrary.org/obo/GAZ_00142030"/>
        <obo:IAO_0000115>A small island on the S rim of the Atufa Atoll.</obo:IAO_0000115>
        <oboInOwl:hasOBONamespace>GAZ</oboInOwl:hasOBONamespace>
        <oboInOwl:id>GAZ:00142063</oboInOwl:id>
        <rdfs:label>Na Hapiti</rdfs:label>
    </owl:NamedIndividual>
    


    <!-- http://purl.obolibrary.org/obo/GAZ_00142064 -->

    <owl:NamedIndividual rdf:about="http://purl.obolibrary.org/obo/GAZ_00142064">
        <obo:RO_0001025 rdf:resource="http://purl.obolibrary.org/obo/GAZ_00142030"/>
        <obo:IAO_0000115>A small island on the S rim of the Atufa Atoll.</obo:IAO_0000115>
        <oboInOwl:hasOBONamespace>GAZ</oboInOwl:hasOBONamespace>
        <oboInOwl:id>GAZ:00142064</oboInOwl:id>
        <rdfs:label>Hakea Lahi i Lalo</rdfs:label>
    </owl:NamedIndividual>
    


    <!-- http://purl.obolibrary.org/obo/GAZ_00142065 -->

    <owl:NamedIndividual rdf:about="http://purl.obolibrary.org/obo/GAZ_00142065">
        <obo:RO_0001025 rdf:resource="http://purl.obolibrary.org/obo/GAZ_00142030"/>
        <obo:IAO_0000115>A small island on the S rim of the Atufa Atoll.</obo:IAO_0000115>
        <oboInOwl:hasOBONamespace>GAZ</oboInOwl:hasOBONamespace>
        <oboInOwl:id>GAZ:00142065</oboInOwl:id>
        <rdfs:label>Hakea O Apelamo</rdfs:label>
    </owl:NamedIndividual>
    


    <!-- http://purl.obolibrary.org/obo/GAZ_00142066 -->

    <owl:NamedIndividual rdf:about="http://purl.obolibrary.org/obo/GAZ_00142066">
        <obo:RO_0001025 rdf:resource="http://purl.obolibrary.org/obo/GAZ_00009562"/>
        <obo:IAO_0000115>The W reef of he Atufu Atoll.</obo:IAO_0000115>
        <oboInOwl:hasOBONamespace>GAZ</oboInOwl:hasOBONamespace>
        <oboInOwl:id>GAZ:00142066</oboInOwl:id>
        <rdfs:label>Te Alofi</rdfs:label>
    </owl:NamedIndividual>
    


    <!-- http://purl.obolibrary.org/obo/GAZ_00142067 -->

    <owl:NamedIndividual rdf:about="http://purl.obolibrary.org/obo/GAZ_00142067">
        <obo:RO_0001025 rdf:resource="http://purl.obolibrary.org/obo/GAZ_00142066"/>
        <obo:IAO_0000115>An island on the W rim of the Atafu Atoll.</obo:IAO_0000115>
        <oboInOwl:hasOBONamespace>GAZ</oboInOwl:hasOBONamespace>
        <oboInOwl:id>GAZ:00142067</oboInOwl:id>
        <rdfs:label>Ulugagie</rdfs:label>
    </owl:NamedIndividual>
    


    <!-- http://purl.obolibrary.org/obo/GAZ_00142068 -->

    <owl:NamedIndividual rdf:about="http://purl.obolibrary.org/obo/GAZ_00142068">
        <obo:RO_0001025 rdf:resource="http://purl.obolibrary.org/obo/GAZ_00142066"/>
        <obo:IAO_0000115>An island on the W rim of the Atafu Atoll.</obo:IAO_0000115>
        <oboInOwl:hasOBONamespace>GAZ</oboInOwl:hasOBONamespace>
        <oboInOwl:id>GAZ:00142068</oboInOwl:id>
        <rdfs:label>Alofi Lahi</rdfs:label>
    </owl:NamedIndividual>
    


    <!-- http://purl.obolibrary.org/obo/GAZ_00142069 -->

    <owl:NamedIndividual rdf:about="http://purl.obolibrary.org/obo/GAZ_00142069">
        <obo:RO_0001025 rdf:resource="http://purl.obolibrary.org/obo/GAZ_00142066"/>
        <obo:IAO_0000115>An island on the W rim of the Atafu Atoll.</obo:IAO_0000115>
        <oboInOwl:hasOBONamespace>GAZ</oboInOwl:hasOBONamespace>
        <oboInOwl:id>GAZ:00142069</oboInOwl:id>
        <rdfs:label>Te Tunoa</rdfs:label>
    </owl:NamedIndividual>
    


    <!-- http://purl.obolibrary.org/obo/GAZ_00142070 -->

    <owl:NamedIndividual rdf:about="http://purl.obolibrary.org/obo/GAZ_00142070">
        <obo:RO_0001025 rdf:resource="http://purl.obolibrary.org/obo/GAZ_00142066"/>
        <obo:IAO_0000115>An island on the W rim of the Atafu Atoll.</obo:IAO_0000115>
        <oboInOwl:hasOBONamespace>GAZ</oboInOwl:hasOBONamespace>
        <oboInOwl:id>GAZ:00142070</oboInOwl:id>
        <rdfs:label>Te Alofi Island</rdfs:label>
    </owl:NamedIndividual>
    


    <!-- http://purl.obolibrary.org/obo/GAZ_00142071 -->

    <owl:NamedIndividual rdf:about="http://purl.obolibrary.org/obo/GAZ_00142071">
        <obo:RO_0001025 rdf:resource="http://purl.obolibrary.org/obo/GAZ_00142066"/>
        <obo:IAO_0000115>An island on the W rim of the Atafu Atoll.</obo:IAO_0000115>
        <oboInOwl:hasOBONamespace>GAZ</oboInOwl:hasOBONamespace>
        <oboInOwl:id>GAZ:00142071</oboInOwl:id>
        <rdfs:label>Folasaga</rdfs:label>
    </owl:NamedIndividual>
    


    <!-- http://purl.obolibrary.org/obo/GAZ_00142072 -->

    <owl:NamedIndividual rdf:about="http://purl.obolibrary.org/obo/GAZ_00142072">
        <obo:RO_0001025 rdf:resource="http://purl.obolibrary.org/obo/GAZ_00142066"/>
        <obo:IAO_0000115>An island on the W rim of the Atafu Atoll.</obo:IAO_0000115>
        <oboInOwl:hasOBONamespace>GAZ</oboInOwl:hasOBONamespace>
        <oboInOwl:id>GAZ:00142072</oboInOwl:id>
        <rdfs:label>Te Puka</rdfs:label>
    </owl:NamedIndividual>
    


    <!-- http://purl.obolibrary.org/obo/GAZ_00142073 -->

    <owl:NamedIndividual rdf:about="http://purl.obolibrary.org/obo/GAZ_00142073">
        <obo:RO_0001025 rdf:resource="http://purl.obolibrary.org/obo/GAZ_00142066"/>
        <obo:IAO_0000115>An island on the W rim of the Atafu Atoll.</obo:IAO_0000115>
        <oboInOwl:hasOBONamespace>GAZ</oboInOwl:hasOBONamespace>
        <oboInOwl:id>GAZ:00142073</oboInOwl:id>
        <rdfs:label>Te Papa Motumotu</rdfs:label>
    </owl:NamedIndividual>
    


    <!-- http://purl.obolibrary.org/obo/GAZ_00142074 -->

    <owl:NamedIndividual rdf:about="http://purl.obolibrary.org/obo/GAZ_00142074">
        <obo:RO_0001025 rdf:resource="http://purl.obolibrary.org/obo/GAZ_00142066"/>
        <obo:IAO_0000115>An island on the W rim of the Atafu Atoll.</obo:IAO_0000115>
        <oboInOwl:hasOBONamespace>GAZ</oboInOwl:hasOBONamespace>
        <oboInOwl:id>GAZ:00142074</oboInOwl:id>
        <rdfs:label>Papa O Tonuia</rdfs:label>
    </owl:NamedIndividual>
    


    <!-- http://purl.obolibrary.org/obo/GAZ_00142075 -->

    <owl:NamedIndividual rdf:about="http://purl.obolibrary.org/obo/GAZ_00142075">
        <obo:RO_0001025 rdf:resource="http://purl.obolibrary.org/obo/GAZ_00142025"/>
        <obo:IAO_0000115>A small island on the N rim of the Atafu Atoll.</obo:IAO_0000115>
        <oboInOwl:hasOBONamespace>GAZ</oboInOwl:hasOBONamespace>
        <oboInOwl:id>GAZ:00142075</oboInOwl:id>
        <rdfs:label>Fogalaki Lalo</rdfs:label>
    </owl:NamedIndividual>
    


    <!-- http://purl.obolibrary.org/obo/GAZ_00142076 -->

    <owl:NamedIndividual rdf:about="http://purl.obolibrary.org/obo/GAZ_00142076">
        <obo:RO_0001025 rdf:resource="http://purl.obolibrary.org/obo/GAZ_00142025"/>
        <obo:IAO_0000115>A small island on the N rim of the Atafu Atoll.</obo:IAO_0000115>
        <oboInOwl:hasOBONamespace>GAZ</oboInOwl:hasOBONamespace>
        <oboInOwl:id>GAZ:00142076</oboInOwl:id>
        <rdfs:label>Fogalaki i Matagi</rdfs:label>
    </owl:NamedIndividual>
    


    <!-- http://purl.obolibrary.org/obo/GAZ_00142077 -->

    <owl:NamedIndividual rdf:about="http://purl.obolibrary.org/obo/GAZ_00142077">
        <obo:RO_0001025 rdf:resource="http://purl.obolibrary.org/obo/GAZ_00142137"/>
        <obo:IAO_0000115>An island on the W rim of the Fakaofo Atoll.</obo:IAO_0000115>
        <oboInOwl:hasOBONamespace>GAZ</oboInOwl:hasOBONamespace>
        <oboInOwl:id>GAZ:00142077</oboInOwl:id>
        <rdfs:label>Fale</rdfs:label>
    </owl:NamedIndividual>
    


    <!-- http://purl.obolibrary.org/obo/GAZ_00142078 -->

    <owl:NamedIndividual rdf:about="http://purl.obolibrary.org/obo/GAZ_00142078">
        <obo:RO_0001025 rdf:resource="http://purl.obolibrary.org/obo/GAZ_00142137"/>
        <obo:IAO_0000115>An island on the SW rim of the Fakaofo Atoll.</obo:IAO_0000115>
        <oboInOwl:hasOBONamespace>GAZ</oboInOwl:hasOBONamespace>
        <oboInOwl:id>GAZ:00142078</oboInOwl:id>
        <rdfs:label>Kauahua O Henua</rdfs:label>
    </owl:NamedIndividual>
    


    <!-- http://purl.obolibrary.org/obo/GAZ_00142079 -->

    <owl:NamedIndividual rdf:about="http://purl.obolibrary.org/obo/GAZ_00142079">
        <obo:RO_0001025 rdf:resource="http://purl.obolibrary.org/obo/GAZ_00142137"/>
        <obo:IAO_0000115>An island on the SW rim of the Fakaofo Atoll.</obo:IAO_0000115>
        <oboInOwl:hasOBONamespace>GAZ</oboInOwl:hasOBONamespace>
        <oboInOwl:id>GAZ:00142079</oboInOwl:id>
        <rdfs:label>Kauahua O Tanifa</rdfs:label>
    </owl:NamedIndividual>
    


    <!-- http://purl.obolibrary.org/obo/GAZ_00142080 -->

    <owl:NamedIndividual rdf:about="http://purl.obolibrary.org/obo/GAZ_00142080">
        <obo:RO_0001025 rdf:resource="http://purl.obolibrary.org/obo/GAZ_00142137"/>
        <obo:IAO_0000115>An island on the SW rim of the Fakaofo Atoll.</obo:IAO_0000115>
        <oboInOwl:hasOBONamespace>GAZ</oboInOwl:hasOBONamespace>
        <oboInOwl:id>GAZ:00142080</oboInOwl:id>
        <rdfs:label>Te Papaloa</rdfs:label>
    </owl:NamedIndividual>
    


    <!-- http://purl.obolibrary.org/obo/GAZ_00142081 -->

    <owl:NamedIndividual rdf:about="http://purl.obolibrary.org/obo/GAZ_00142081">
        <obo:RO_0001025 rdf:resource="http://purl.obolibrary.org/obo/GAZ_00142137"/>
        <obo:IAO_0000115>An island on the SW rim of the Fakaofo Atoll.</obo:IAO_0000115>
        <oboInOwl:hasOBONamespace>GAZ</oboInOwl:hasOBONamespace>
        <oboInOwl:id>GAZ:00142081</oboInOwl:id>
        <rdfs:label>Kauahua Uli</rdfs:label>
    </owl:NamedIndividual>
    


    <!-- http://purl.obolibrary.org/obo/GAZ_00142082 -->

    <owl:NamedIndividual rdf:about="http://purl.obolibrary.org/obo/GAZ_00142082">
        <obo:RO_0001025 rdf:resource="http://purl.obolibrary.org/obo/GAZ_00142137"/>
        <obo:IAO_0000115>An island on the SW rim of the Fakaofo Atoll.</obo:IAO_0000115>
        <oboInOwl:hasOBONamespace>GAZ</oboInOwl:hasOBONamespace>
        <oboInOwl:id>GAZ:00142082</oboInOwl:id>
        <rdfs:label>Kauahua O Kupega</rdfs:label>
    </owl:NamedIndividual>
    


    <!-- http://purl.obolibrary.org/obo/GAZ_00142083 -->

    <owl:NamedIndividual rdf:about="http://purl.obolibrary.org/obo/GAZ_00142083">
        <obo:RO_0001025 rdf:resource="http://purl.obolibrary.org/obo/GAZ_00142132"/>
        <obo:IAO_0000115>An island on the SE rim of the Fakaofo Atoll.</obo:IAO_0000115>
        <oboInOwl:hasOBONamespace>GAZ</oboInOwl:hasOBONamespace>
        <oboInOwl:id>GAZ:00142083</oboInOwl:id>
        <rdfs:label>Hakea</rdfs:label>
    </owl:NamedIndividual>
    


    <!-- http://purl.obolibrary.org/obo/GAZ_00142084 -->

    <owl:NamedIndividual rdf:about="http://purl.obolibrary.org/obo/GAZ_00142084">
        <obo:RO_0001025 rdf:resource="http://purl.obolibrary.org/obo/GAZ_00142137"/>
        <obo:IAO_0000115>An island on the SW rim of the Fakaofo Atoll.</obo:IAO_0000115>
        <oboInOwl:hasOBONamespace>GAZ</oboInOwl:hasOBONamespace>
        <oboInOwl:id>GAZ:00142084</oboInOwl:id>
        <rdfs:label>Te Kau alua O Humu</rdfs:label>
    </owl:NamedIndividual>
    


    <!-- http://purl.obolibrary.org/obo/GAZ_00142085 -->

    <owl:NamedIndividual rdf:about="http://purl.obolibrary.org/obo/GAZ_00142085">
        <obo:RO_0001025 rdf:resource="http://purl.obolibrary.org/obo/GAZ_00142132"/>
        <obo:IAO_0000115>An island on the E rim of the Fakaofo Atoll.</obo:IAO_0000115>
        <oboInOwl:hasOBONamespace>GAZ</oboInOwl:hasOBONamespace>
        <oboInOwl:id>GAZ:00142085</oboInOwl:id>
        <rdfs:label>Tafulaelo</rdfs:label>
    </owl:NamedIndividual>
    


    <!-- http://purl.obolibrary.org/obo/GAZ_00142086 -->

    <owl:NamedIndividual rdf:about="http://purl.obolibrary.org/obo/GAZ_00142086">
        <obo:RO_0001025 rdf:resource="http://purl.obolibrary.org/obo/GAZ_00142137"/>
        <obo:IAO_0000115>The most W of the islands of the Fakaofo Atoll.</obo:IAO_0000115>
        <oboInOwl:hasOBONamespace>GAZ</oboInOwl:hasOBONamespace>
        <oboInOwl:id>GAZ:00142086</oboInOwl:id>
        <rdfs:label>Fenua Fala</rdfs:label>
    </owl:NamedIndividual>
    


    <!-- http://purl.obolibrary.org/obo/GAZ_00142087 -->

    <owl:NamedIndividual rdf:about="http://purl.obolibrary.org/obo/GAZ_00142087">
        <obo:RO_0001025 rdf:resource="http://purl.obolibrary.org/obo/GAZ_00142135"/>
        <obo:IAO_0000115>An island on the E rim of the Fakaofo Atoll.</obo:IAO_0000115>
        <oboInOwl:hasOBONamespace>GAZ</oboInOwl:hasOBONamespace>
        <oboInOwl:id>GAZ:00142087</oboInOwl:id>
        <rdfs:label>Te Loto</rdfs:label>
    </owl:NamedIndividual>
    


    <!-- http://purl.obolibrary.org/obo/GAZ_00142088 -->

    <owl:NamedIndividual rdf:about="http://purl.obolibrary.org/obo/GAZ_00142088">
        <obo:RO_0001025 rdf:resource="http://purl.obolibrary.org/obo/GAZ_00142132"/>
        <obo:IAO_0000115>An island on the E rim of the Fakaofo Atoll.</obo:IAO_0000115>
        <oboInOwl:hasOBONamespace>GAZ</oboInOwl:hasOBONamespace>
        <oboInOwl:id>GAZ:00142088</oboInOwl:id>
        <rdfs:label>Pagai</rdfs:label>
    </owl:NamedIndividual>
    


    <!-- http://purl.obolibrary.org/obo/GAZ_00142089 -->

    <owl:NamedIndividual rdf:about="http://purl.obolibrary.org/obo/GAZ_00142089">
        <obo:RO_0001025 rdf:resource="http://purl.obolibrary.org/obo/GAZ_00142132"/>
        <obo:IAO_0000115>An island on the E rim of the Fakaofo Atoll.</obo:IAO_0000115>
        <oboInOwl:hasOBONamespace>GAZ</oboInOwl:hasOBONamespace>
        <oboInOwl:id>GAZ:00142089</oboInOwl:id>
        <rdfs:label>Falatutahi</rdfs:label>
    </owl:NamedIndividual>
    


    <!-- http://purl.obolibrary.org/obo/GAZ_00142090 -->

    <owl:NamedIndividual rdf:about="http://purl.obolibrary.org/obo/GAZ_00142090">
        <obo:RO_0001025 rdf:resource="http://purl.obolibrary.org/obo/GAZ_00142132"/>
        <obo:IAO_0000115>An island on the E rim of the Fakaofo Atoll.</obo:IAO_0000115>
        <oboInOwl:hasOBONamespace>GAZ</oboInOwl:hasOBONamespace>
        <oboInOwl:id>GAZ:00142090</oboInOwl:id>
        <rdfs:label>Motuloa</rdfs:label>
    </owl:NamedIndividual>
    


    <!-- http://purl.obolibrary.org/obo/GAZ_00142091 -->

    <owl:NamedIndividual rdf:about="http://purl.obolibrary.org/obo/GAZ_00142091">
        <obo:RO_0001025 rdf:resource="http://purl.obolibrary.org/obo/GAZ_00142131"/>
        <obo:IAO_0000115>An island on the NE rim of the Fakaofo Atoll.</obo:IAO_0000115>
        <oboInOwl:hasOBONamespace>GAZ</oboInOwl:hasOBONamespace>
        <oboInOwl:id>GAZ:00142091</oboInOwl:id>
        <rdfs:label>Te Lafu</rdfs:label>
    </owl:NamedIndividual>
    


    <!-- http://purl.obolibrary.org/obo/GAZ_00142092 -->

    <owl:NamedIndividual rdf:about="http://purl.obolibrary.org/obo/GAZ_00142092">
        <obo:RO_0001025 rdf:resource="http://purl.obolibrary.org/obo/GAZ_00142125"/>
        <obo:IAO_0000115>An island on the W of the Nukunonu Atoll.</obo:IAO_0000115>
        <oboInOwl:hasOBONamespace>GAZ</oboInOwl:hasOBONamespace>
        <oboInOwl:id>GAZ:00142092</oboInOwl:id>
        <rdfs:label>Te Tauhunu</rdfs:label>
    </owl:NamedIndividual>
    


    <!-- http://purl.obolibrary.org/obo/GAZ_00142093 -->

    <owl:NamedIndividual rdf:about="http://purl.obolibrary.org/obo/GAZ_00142093">
        <obo:RO_0001025 rdf:resource="http://purl.obolibrary.org/obo/GAZ_00142120"/>
        <obo:IAO_0000115>An island on the S of the Nukunonu Atoll.</obo:IAO_0000115>
        <oboInOwl:hasOBONamespace>GAZ</oboInOwl:hasOBONamespace>
        <oboInOwl:id>GAZ:00142093</oboInOwl:id>
        <rdfs:label>Te Afua</rdfs:label>
    </owl:NamedIndividual>
    


    <!-- http://purl.obolibrary.org/obo/GAZ_00142094 -->

    <owl:NamedIndividual rdf:about="http://purl.obolibrary.org/obo/GAZ_00142094">
        <obo:RO_0001025 rdf:resource="http://purl.obolibrary.org/obo/GAZ_00142120"/>
        <obo:IAO_0000115>An island on the S of the Nukunonu Atoll.</obo:IAO_0000115>
        <oboInOwl:hasOBONamespace>GAZ</oboInOwl:hasOBONamespace>
        <oboInOwl:id>GAZ:00142094</oboInOwl:id>
        <rdfs:label>Kauafa a Kele</rdfs:label>
    </owl:NamedIndividual>
    


    <!-- http://purl.obolibrary.org/obo/GAZ_00142095 -->

    <owl:NamedIndividual rdf:about="http://purl.obolibrary.org/obo/GAZ_00142095">
        <obo:RO_0001025 rdf:resource="http://purl.obolibrary.org/obo/GAZ_00142120"/>
        <obo:IAO_0000115>An island on the S of the Nukunonu Atoll.</obo:IAO_0000115>
        <oboInOwl:hasOBONamespace>GAZ</oboInOwl:hasOBONamespace>
        <oboInOwl:id>GAZ:00142095</oboInOwl:id>
        <rdfs:label>Na Hapati</rdfs:label>
    </owl:NamedIndividual>
    


    <!-- http://purl.obolibrary.org/obo/GAZ_00142096 -->

    <owl:NamedIndividual rdf:about="http://purl.obolibrary.org/obo/GAZ_00142096">
        <obo:RO_0001025 rdf:resource="http://purl.obolibrary.org/obo/GAZ_00142120"/>
        <obo:IAO_0000115>An island on the S of the Nukunonu Atoll.</obo:IAO_0000115>
        <oboInOwl:hasOBONamespace>GAZ</oboInOwl:hasOBONamespace>
        <oboInOwl:id>GAZ:00142096</oboInOwl:id>
        <rdfs:label>Motua Akea</rdfs:label>
    </owl:NamedIndividual>
    


    <!-- http://purl.obolibrary.org/obo/GAZ_00142097 -->

    <owl:NamedIndividual rdf:about="http://purl.obolibrary.org/obo/GAZ_00142097">
        <obo:RO_0001025 rdf:resource="http://purl.obolibrary.org/obo/GAZ_00142120"/>
        <obo:IAO_0000115>An island on the S of the Nukunonu Atoll.</obo:IAO_0000115>
        <oboInOwl:hasOBONamespace>GAZ</oboInOwl:hasOBONamespace>
        <oboInOwl:id>GAZ:00142097</oboInOwl:id>
        <rdfs:label>Na Papa [South]</rdfs:label>
    </owl:NamedIndividual>
    


    <!-- http://purl.obolibrary.org/obo/GAZ_00142098 -->

    <owl:NamedIndividual rdf:about="http://purl.obolibrary.org/obo/GAZ_00142098">
        <obo:RO_0001025 rdf:resource="http://purl.obolibrary.org/obo/GAZ_00142120"/>
        <obo:IAO_0000115>An island on the SS of the Nukunonu Atoll.</obo:IAO_0000115>
        <oboInOwl:hasOBONamespace>GAZ</oboInOwl:hasOBONamespace>
        <oboInOwl:id>GAZ:00142098</oboInOwl:id>
        <rdfs:label>Na Papa o Atawhu</rdfs:label>
    </owl:NamedIndividual>
    


    <!-- http://purl.obolibrary.org/obo/GAZ_00142099 -->

    <owl:NamedIndividual rdf:about="http://purl.obolibrary.org/obo/GAZ_00142099">
        <obo:RO_0001025 rdf:resource="http://purl.obolibrary.org/obo/GAZ_00142120"/>
        <obo:IAO_0000115>An island on the SW of the Nukunonu Atoll, S of Nukunonu.</obo:IAO_0000115>
        <oboInOwl:hasOBONamespace>GAZ</oboInOwl:hasOBONamespace>
        <oboInOwl:id>GAZ:00142099</oboInOwl:id>
        <rdfs:label>Na Papa [West]</rdfs:label>
    </owl:NamedIndividual>
    


    <!-- http://purl.obolibrary.org/obo/GAZ_00142100 -->

    <owl:NamedIndividual rdf:about="http://purl.obolibrary.org/obo/GAZ_00142100">
        <obo:RO_0001025 rdf:resource="http://purl.obolibrary.org/obo/GAZ_00142120"/>
        <obo:IAO_0000115>An island on the SW of the Nukunonu Atoll.</obo:IAO_0000115>
        <oboInOwl:hasOBONamespace>GAZ</oboInOwl:hasOBONamespace>
        <oboInOwl:id>GAZ:00142100</oboInOwl:id>
        <rdfs:label>Nahau</rdfs:label>
    </owl:NamedIndividual>
    


    <!-- http://purl.obolibrary.org/obo/GAZ_00142101 -->

    <owl:NamedIndividual rdf:about="http://purl.obolibrary.org/obo/GAZ_00142101">
        <obo:RO_0001025 rdf:resource="http://purl.obolibrary.org/obo/GAZ_00142120"/>
        <obo:IAO_0000115>An island on the S of the Nukunonu Atoll.</obo:IAO_0000115>
        <oboInOwl:hasOBONamespace>GAZ</oboInOwl:hasOBONamespace>
        <oboInOwl:id>GAZ:00142101</oboInOwl:id>
        <rdfs:label>Fulumahaga</rdfs:label>
    </owl:NamedIndividual>
    


    <!-- http://purl.obolibrary.org/obo/GAZ_00142102 -->

    <owl:NamedIndividual rdf:about="http://purl.obolibrary.org/obo/GAZ_00142102">
        <obo:RO_0001025 rdf:resource="http://purl.obolibrary.org/obo/GAZ_00142113"/>
        <obo:IAO_0000115>An island on the E of the Nukunonu Atoll.</obo:IAO_0000115>
        <oboInOwl:hasOBONamespace>GAZ</oboInOwl:hasOBONamespace>
        <oboInOwl:id>GAZ:00142102</oboInOwl:id>
        <rdfs:label>Tagamako</rdfs:label>
    </owl:NamedIndividual>
    


    <!-- http://purl.obolibrary.org/obo/GAZ_00142103 -->

    <owl:NamedIndividual rdf:about="http://purl.obolibrary.org/obo/GAZ_00142103">
        <obo:RO_0001025 rdf:resource="http://purl.obolibrary.org/obo/GAZ_00142113"/>
        <obo:IAO_0000115>An island on the E of the Nukunonu Atoll.</obo:IAO_0000115>
        <oboInOwl:hasOBONamespace>GAZ</oboInOwl:hasOBONamespace>
        <oboInOwl:id>GAZ:00142103</oboInOwl:id>
        <rdfs:label>Olomoana</rdfs:label>
    </owl:NamedIndividual>
    


    <!-- http://purl.obolibrary.org/obo/GAZ_00142104 -->

    <owl:NamedIndividual rdf:about="http://purl.obolibrary.org/obo/GAZ_00142104">
        <obo:RO_0001025 rdf:resource="http://purl.obolibrary.org/obo/GAZ_00142117"/>
        <obo:IAO_0000115>An island on the W of Nukunonu Atoll.</obo:IAO_0000115>
        <oboInOwl:hasOBONamespace>GAZ</oboInOwl:hasOBONamespace>
        <oboInOwl:id>GAZ:00142104</oboInOwl:id>
        <rdfs:label>Fakanava tau loto</rdfs:label>
    </owl:NamedIndividual>
    


    <!-- http://purl.obolibrary.org/obo/GAZ_00142105 -->

    <owl:NamedIndividual rdf:about="http://purl.obolibrary.org/obo/GAZ_00142105">
        <obo:RO_0001025 rdf:resource="http://purl.obolibrary.org/obo/GAZ_00142113"/>
        <obo:IAO_0000115>An island on the E of the Nukunonu Atoll.</obo:IAO_0000115>
        <oboInOwl:hasOBONamespace>GAZ</oboInOwl:hasOBONamespace>
        <oboInOwl:id>GAZ:00142105</oboInOwl:id>
        <rdfs:label>Lalohumu</rdfs:label>
    </owl:NamedIndividual>
    


    <!-- http://purl.obolibrary.org/obo/GAZ_00142106 -->

    <owl:NamedIndividual rdf:about="http://purl.obolibrary.org/obo/GAZ_00142106">
        <obo:RO_0001025 rdf:resource="http://purl.obolibrary.org/obo/GAZ_00142113"/>
        <obo:IAO_0000115>An island on the E of the Nukunonu Atoll.</obo:IAO_0000115>
        <oboInOwl:hasOBONamespace>GAZ</oboInOwl:hasOBONamespace>
        <oboInOwl:id>GAZ:00142106</oboInOwl:id>
        <rdfs:label>Vaivaimai</rdfs:label>
    </owl:NamedIndividual>
    


    <!-- http://purl.obolibrary.org/obo/GAZ_00142107 -->

    <owl:NamedIndividual rdf:about="http://purl.obolibrary.org/obo/GAZ_00142107">
        <obo:RO_0001025 rdf:resource="http://purl.obolibrary.org/obo/GAZ_00142113"/>
        <obo:IAO_0000115>An island on the E of the Nukunonu Atoll.</obo:IAO_0000115>
        <oboInOwl:hasOBONamespace>GAZ</oboInOwl:hasOBONamespace>
        <oboInOwl:id>GAZ:00142107</oboInOwl:id>
        <rdfs:label>Te Palaoa</rdfs:label>
    </owl:NamedIndividual>
    


    <!-- http://purl.obolibrary.org/obo/GAZ_00142108 -->

    <owl:NamedIndividual rdf:about="http://purl.obolibrary.org/obo/GAZ_00142108">
        <obo:RO_0001025 rdf:resource="http://purl.obolibrary.org/obo/GAZ_00142113"/>
        <obo:IAO_0000115>An island on the E of the Nukunonu Atoll.</obo:IAO_0000115>
        <oboInOwl:hasOBONamespace>GAZ</oboInOwl:hasOBONamespace>
        <oboInOwl:id>GAZ:00142108</oboInOwl:id>
        <rdfs:label>Te Nonu</rdfs:label>
    </owl:NamedIndividual>
    


    <!-- http://purl.obolibrary.org/obo/GAZ_00142109 -->

    <owl:NamedIndividual rdf:about="http://purl.obolibrary.org/obo/GAZ_00142109">
        <obo:RO_0001025 rdf:resource="http://purl.obolibrary.org/obo/GAZ_00142113"/>
        <obo:IAO_0000115>An island on the E of the Nukunonu Atoll.</obo:IAO_0000115>
        <oboInOwl:hasOBONamespace>GAZ</oboInOwl:hasOBONamespace>
        <oboInOwl:id>GAZ:00142109</oboInOwl:id>
        <rdfs:label>Hilakehe</rdfs:label>
    </owl:NamedIndividual>
    


    <!-- http://purl.obolibrary.org/obo/GAZ_00142110 -->

    <owl:NamedIndividual rdf:about="http://purl.obolibrary.org/obo/GAZ_00142110">
        <obo:RO_0001025 rdf:resource="http://purl.obolibrary.org/obo/GAZ_00142111"/>
        <obo:IAO_0000115>Islands on the N rim of the Nukunonu Atoll.</obo:IAO_0000115>
        <oboInOwl:hasOBONamespace>GAZ</oboInOwl:hasOBONamespace>
        <oboInOwl:id>GAZ:00142110</oboInOwl:id>
        <rdfs:label>Na Kaupapa</rdfs:label>
    </owl:NamedIndividual>
    


    <!-- http://purl.obolibrary.org/obo/GAZ_00142111 -->

    <owl:NamedIndividual rdf:about="http://purl.obolibrary.org/obo/GAZ_00142111">
        <obo:RO_0001025 rdf:resource="http://purl.obolibrary.org/obo/GAZ_00009560"/>
        <obo:IAO_0000115>The N reef of the Nukunonu Atoll.</obo:IAO_0000115>
        <oboInOwl:hasOBONamespace>GAZ</oboInOwl:hasOBONamespace>
        <oboInOwl:id>GAZ:00142111</oboInOwl:id>
        <rdfs:label>Ahaga Loa</rdfs:label>
    </owl:NamedIndividual>
    


    <!-- http://purl.obolibrary.org/obo/GAZ_00142112 -->

    <owl:NamedIndividual rdf:about="http://purl.obolibrary.org/obo/GAZ_00142112">
        <obo:RO_0001025 rdf:resource="http://purl.obolibrary.org/obo/GAZ_00142119"/>
        <obo:IAO_0000115>A long island at the SE of the Nukunonu Atoll, apparently unamed.</obo:IAO_0000115>
        <oboInOwl:hasOBONamespace>GAZ</oboInOwl:hasOBONamespace>
        <oboInOwl:id>GAZ:00142112</oboInOwl:id>
        <rdfs:label>Unamed Island</rdfs:label>
    </owl:NamedIndividual>
    


    <!-- http://purl.obolibrary.org/obo/GAZ_00142113 -->

    <owl:NamedIndividual rdf:about="http://purl.obolibrary.org/obo/GAZ_00142113">
        <obo:RO_0001025 rdf:resource="http://purl.obolibrary.org/obo/GAZ_00009560"/>
        <obo:IAO_0000115>The E reef of the Nukunonu Atoll.</obo:IAO_0000115>
        <oboInOwl:hasOBONamespace>GAZ</oboInOwl:hasOBONamespace>
        <oboInOwl:id>GAZ:00142113</oboInOwl:id>
        <rdfs:label>Te Kavakava</rdfs:label>
    </owl:NamedIndividual>
    


    <!-- http://purl.obolibrary.org/obo/GAZ_00142114 -->

    <owl:NamedIndividual rdf:about="http://purl.obolibrary.org/obo/GAZ_00142114">
        <obo:RO_0001025 rdf:resource="http://purl.obolibrary.org/obo/GAZ_00142113"/>
        <obo:IAO_0000115>An island on the E of the Nukunonu Atoll.</obo:IAO_0000115>
        <oboInOwl:hasOBONamespace>GAZ</oboInOwl:hasOBONamespace>
        <oboInOwl:id>GAZ:00142114</oboInOwl:id>
        <rdfs:label>Tuigaika</rdfs:label>
    </owl:NamedIndividual>
    


    <!-- http://purl.obolibrary.org/obo/GAZ_00142115 -->

    <owl:NamedIndividual rdf:about="http://purl.obolibrary.org/obo/GAZ_00142115">
        <obo:RO_0001025 rdf:resource="http://purl.obolibrary.org/obo/GAZ_00142113"/>
        <obo:IAO_0000115>An island on the E of the Nukunonu Atoll.</obo:IAO_0000115>
        <oboInOwl:hasOBONamespace>GAZ</oboInOwl:hasOBONamespace>
        <oboInOwl:id>GAZ:00142115</oboInOwl:id>
        <rdfs:label>Haumagalu</rdfs:label>
    </owl:NamedIndividual>
    


    <!-- http://purl.obolibrary.org/obo/GAZ_00142116 -->

    <owl:NamedIndividual rdf:about="http://purl.obolibrary.org/obo/GAZ_00142116">
        <obo:RO_0001025 rdf:resource="http://purl.obolibrary.org/obo/GAZ_00142113"/>
        <obo:IAO_0000115>An island on the E of the Nukunonu Atoll.</obo:IAO_0000115>
        <oboInOwl:hasOBONamespace>GAZ</oboInOwl:hasOBONamespace>
        <oboInOwl:id>GAZ:00142116</oboInOwl:id>
        <rdfs:label>Tima</rdfs:label>
    </owl:NamedIndividual>
    


    <!-- http://purl.obolibrary.org/obo/GAZ_00142117 -->

    <owl:NamedIndividual rdf:about="http://purl.obolibrary.org/obo/GAZ_00142117">
        <obo:RO_0001025 rdf:resource="http://purl.obolibrary.org/obo/GAZ_00009560"/>
        <obo:IAO_0000115>The W reef of the Nukunonu Atoll.</obo:IAO_0000115>
        <oboInOwl:hasOBONamespace>GAZ</oboInOwl:hasOBONamespace>
        <oboInOwl:id>GAZ:00142117</oboInOwl:id>
        <rdfs:label>Te Alofi</rdfs:label>
    </owl:NamedIndividual>
    


    <!-- http://purl.obolibrary.org/obo/GAZ_00142118 -->

    <owl:NamedIndividual rdf:about="http://purl.obolibrary.org/obo/GAZ_00142118">
        <obo:RO_0001025 rdf:resource="http://purl.obolibrary.org/obo/GAZ_00142117"/>
        <oboInOwl:hasOBONamespace>GAZ</oboInOwl:hasOBONamespace>
        <oboInOwl:id>GAZ:00142118</oboInOwl:id>
        <rdfs:label>Te Puka i Muli</rdfs:label>
    </owl:NamedIndividual>
    


    <!-- http://purl.obolibrary.org/obo/GAZ_00142119 -->

    <owl:NamedIndividual rdf:about="http://purl.obolibrary.org/obo/GAZ_00142119">
        <obo:RO_0001025 rdf:resource="http://purl.obolibrary.org/obo/GAZ_00009560"/>
        <obo:IAO_0000115>The SE reef of the Nukunonu Atoll.</obo:IAO_0000115>
        <oboInOwl:hasOBONamespace>GAZ</oboInOwl:hasOBONamespace>
        <oboInOwl:id>GAZ:00142119</oboInOwl:id>
        <rdfs:label>Lalo Na Taulaga</rdfs:label>
    </owl:NamedIndividual>
    


    <!-- http://purl.obolibrary.org/obo/GAZ_00142120 -->

    <owl:NamedIndividual rdf:about="http://purl.obolibrary.org/obo/GAZ_00142120">
        <obo:RO_0001025 rdf:resource="http://purl.obolibrary.org/obo/GAZ_00009560"/>
        <obo:IAO_0000115>The S and SW reef of the Nukunonu Atoll.</obo:IAO_0000115>
        <oboInOwl:hasOBONamespace>GAZ</oboInOwl:hasOBONamespace>
        <oboInOwl:id>GAZ:00142120</oboInOwl:id>
        <rdfs:label>Te Atu Motu</rdfs:label>
    </owl:NamedIndividual>
    


    <!-- http://purl.obolibrary.org/obo/GAZ_00142121 -->

    <owl:NamedIndividual rdf:about="http://purl.obolibrary.org/obo/GAZ_00142121">
        <obo:RO_0001025 rdf:resource="http://purl.obolibrary.org/obo/GAZ_00009560"/>
        <obo:IAO_0000115>The SE reef of Nukunonu Atoll.</obo:IAO_0000115>
        <oboInOwl:hasOBONamespace>GAZ</oboInOwl:hasOBONamespace>
        <oboInOwl:id>GAZ:00142121</oboInOwl:id>
        <rdfs:label>Vaitupu</rdfs:label>
    </owl:NamedIndividual>
    


    <!-- http://purl.obolibrary.org/obo/GAZ_00142122 -->

    <owl:NamedIndividual rdf:about="http://purl.obolibrary.org/obo/GAZ_00142122">
        <obo:RO_0001025 rdf:resource="http://purl.obolibrary.org/obo/GAZ_00142121"/>
        <obo:IAO_0000115>An island on the SE of the Nukunonu Atoll.</obo:IAO_0000115>
        <oboInOwl:hasOBONamespace>GAZ</oboInOwl:hasOBONamespace>
        <oboInOwl:id>GAZ:00142122</oboInOwl:id>
        <rdfs:label>Niu Whoawhoa</rdfs:label>
    </owl:NamedIndividual>
    


    <!-- http://purl.obolibrary.org/obo/GAZ_00142123 -->

    <owl:NamedIndividual rdf:about="http://purl.obolibrary.org/obo/GAZ_00142123">
        <obo:RO_0001025 rdf:resource="http://purl.obolibrary.org/obo/GAZ_00142120"/>
        <obo:IAO_0000115>An island in the SW of the Nukunonu Atoll.</obo:IAO_0000115>
        <oboInOwl:hasOBONamespace>GAZ</oboInOwl:hasOBONamespace>
        <oboInOwl:id>GAZ:00142123</oboInOwl:id>
        <rdfs:label>Te Mata Papa</rdfs:label>
    </owl:NamedIndividual>
    


    <!-- http://purl.obolibrary.org/obo/GAZ_00142124 -->

    <owl:NamedIndividual rdf:about="http://purl.obolibrary.org/obo/GAZ_00142124">
        <obo:RO_0001025 rdf:resource="http://purl.obolibrary.org/obo/GAZ_00009560"/>
        <obo:IAO_0000115>A W reef of the Nukunonu Atoll.</obo:IAO_0000115>
        <oboInOwl:hasOBONamespace>GAZ</oboInOwl:hasOBONamespace>
        <oboInOwl:id>GAZ:00142124</oboInOwl:id>
        <rdfs:label>Te Ahaga Lahi</rdfs:label>
    </owl:NamedIndividual>
    


    <!-- http://purl.obolibrary.org/obo/GAZ_00142125 -->

    <owl:NamedIndividual rdf:about="http://purl.obolibrary.org/obo/GAZ_00142125">
        <obo:RO_0001025 rdf:resource="http://purl.obolibrary.org/obo/GAZ_00009560"/>
        <obo:IAO_0000115>A W reef of the Nukunonu Atoll.</obo:IAO_0000115>
        <oboInOwl:hasOBONamespace>GAZ</oboInOwl:hasOBONamespace>
        <oboInOwl:id>GAZ:00142125</oboInOwl:id>
        <rdfs:label>Te Ahaga Likiliki</rdfs:label>
    </owl:NamedIndividual>
    


    <!-- http://purl.obolibrary.org/obo/GAZ_00142126 -->

    <owl:NamedIndividual rdf:about="http://purl.obolibrary.org/obo/GAZ_00142126">
        <obo:RO_0001025 rdf:resource="http://purl.obolibrary.org/obo/GAZ_00142113"/>
        <obo:IAO_0000115>An island on the E of the Nukunonu Atoll.</obo:IAO_0000115>
        <oboInOwl:hasOBONamespace>GAZ</oboInOwl:hasOBONamespace>
        <oboInOwl:id>GAZ:00142126</oboInOwl:id>
        <rdfs:label>Tuatiga</rdfs:label>
    </owl:NamedIndividual>
    


    <!-- http://purl.obolibrary.org/obo/GAZ_00142127 -->

    <owl:NamedIndividual rdf:about="http://purl.obolibrary.org/obo/GAZ_00142127">
        <obo:RO_0001025 rdf:resource="http://purl.obolibrary.org/obo/GAZ_00142113"/>
        <obo:IAO_0000115>An island on the E of the Nukunonu Atoll.</obo:IAO_0000115>
        <oboInOwl:hasOBONamespace>GAZ</oboInOwl:hasOBONamespace>
        <oboInOwl:id>GAZ:00142127</oboInOwl:id>
        <rdfs:label>Niualemu</rdfs:label>
    </owl:NamedIndividual>
    


    <!-- http://purl.obolibrary.org/obo/GAZ_00142128 -->

    <owl:NamedIndividual rdf:about="http://purl.obolibrary.org/obo/GAZ_00142128">
        <obo:RO_0001025 rdf:resource="http://purl.obolibrary.org/obo/GAZ_00142113"/>
        <obo:IAO_0000115>An island on the E of the Nukunonu Atoll.</obo:IAO_0000115>
        <oboInOwl:hasOBONamespace>GAZ</oboInOwl:hasOBONamespace>
        <oboInOwl:id>GAZ:00142128</oboInOwl:id>
        <rdfs:label>Matalapa</rdfs:label>
    </owl:NamedIndividual>
    


    <!-- http://purl.obolibrary.org/obo/GAZ_00142129 -->

    <owl:NamedIndividual rdf:about="http://purl.obolibrary.org/obo/GAZ_00142129">
        <obo:RO_0001025 rdf:resource="http://purl.obolibrary.org/obo/GAZ_00142113"/>
        <obo:IAO_0000115>An island on the E of the Nukunonu Atoll.</obo:IAO_0000115>
        <oboInOwl:hasOBONamespace>GAZ</oboInOwl:hasOBONamespace>
        <oboInOwl:id>GAZ:00142129</oboInOwl:id>
        <rdfs:label>Hini Ailini</rdfs:label>
    </owl:NamedIndividual>
    


    <!-- http://purl.obolibrary.org/obo/GAZ_00142130 -->

    <owl:NamedIndividual rdf:about="http://purl.obolibrary.org/obo/GAZ_00142130">
        <obo:RO_0001025 rdf:resource="http://purl.obolibrary.org/obo/GAZ_00142113"/>
        <obo:IAO_0000115>An island on the E of the Nukunonu Atoll.</obo:IAO_0000115>
        <oboInOwl:hasOBONamespace>GAZ</oboInOwl:hasOBONamespace>
        <oboInOwl:id>GAZ:00142130</oboInOwl:id>
        <rdfs:label>Patuki</rdfs:label>
    </owl:NamedIndividual>
    


    <!-- http://purl.obolibrary.org/obo/GAZ_00142131 -->

    <owl:NamedIndividual rdf:about="http://purl.obolibrary.org/obo/GAZ_00142131">
        <obo:RO_0001025 rdf:resource="http://purl.obolibrary.org/obo/GAZ_00009561"/>
        <obo:IAO_0000115>The NE reef of the Fakaofo Atoll.</obo:IAO_0000115>
        <oboInOwl:hasOBONamespace>GAZ</oboInOwl:hasOBONamespace>
        <oboInOwl:id>GAZ:00142131</oboInOwl:id>
        <rdfs:label>Te Lafu</rdfs:label>
    </owl:NamedIndividual>
    


    <!-- http://purl.obolibrary.org/obo/GAZ_00142132 -->

    <owl:NamedIndividual rdf:about="http://purl.obolibrary.org/obo/GAZ_00142132">
        <obo:RO_0001025 rdf:resource="http://purl.obolibrary.org/obo/GAZ_00009561"/>
        <obo:IAO_0000115>The E reef of the Fakaofo Atoll.</obo:IAO_0000115>
        <oboInOwl:hasOBONamespace>GAZ</oboInOwl:hasOBONamespace>
        <oboInOwl:id>GAZ:00142132</oboInOwl:id>
        <rdfs:label>Te Atu Motu</rdfs:label>
    </owl:NamedIndividual>
    


    <!-- http://purl.obolibrary.org/obo/GAZ_00142133 -->

    <owl:NamedIndividual rdf:about="http://purl.obolibrary.org/obo/GAZ_00142133">
        <obo:RO_0001025 rdf:resource="http://purl.obolibrary.org/obo/GAZ_00009561"/>
        <obo:IAO_0000115>The NW reef of the Fakaofo Atoll.</obo:IAO_0000115>
        <oboInOwl:hasOBONamespace>GAZ</oboInOwl:hasOBONamespace>
        <oboInOwl:id>GAZ:00142133</oboInOwl:id>
        <rdfs:label>Ahaga Loa</rdfs:label>
    </owl:NamedIndividual>
    


    <!-- http://purl.obolibrary.org/obo/GAZ_00142134 -->

    <owl:NamedIndividual rdf:about="http://purl.obolibrary.org/obo/GAZ_00142134">
        <obo:RO_0001025 rdf:resource="http://purl.obolibrary.org/obo/GAZ_00009561"/>
        <obo:IAO_0000115>The E reef of the Fakaofo Atoll.</obo:IAO_0000115>
        <oboInOwl:hasOBONamespace>GAZ</oboInOwl:hasOBONamespace>
        <oboInOwl:id>GAZ:00142134</oboInOwl:id>
        <rdfs:label>Te Tu Fa</rdfs:label>
    </owl:NamedIndividual>
    


    <!-- http://purl.obolibrary.org/obo/GAZ_00142135 -->

    <owl:NamedIndividual rdf:about="http://purl.obolibrary.org/obo/GAZ_00142135">
        <obo:RO_0001025 rdf:resource="http://purl.obolibrary.org/obo/GAZ_00009561"/>
        <obo:IAO_0000115>A SE reef of the Fakaofo Atoll, N of Te Atu Hakea.</obo:IAO_0000115>
        <oboInOwl:hasOBONamespace>GAZ</oboInOwl:hasOBONamespace>
        <oboInOwl:id>GAZ:00142135</oboInOwl:id>
        <rdfs:label>Te Loto</rdfs:label>
    </owl:NamedIndividual>
    


    <!-- http://purl.obolibrary.org/obo/GAZ_00142136 -->

    <owl:NamedIndividual rdf:about="http://purl.obolibrary.org/obo/GAZ_00142136">
        <obo:RO_0001025 rdf:resource="http://purl.obolibrary.org/obo/GAZ_00009561"/>
        <obo:IAO_0000115>The SE reef of the Fakaofo Atoll.</obo:IAO_0000115>
        <oboInOwl:hasOBONamespace>GAZ</oboInOwl:hasOBONamespace>
        <oboInOwl:id>GAZ:00142136</oboInOwl:id>
        <rdfs:label>Te Atu Hakea</rdfs:label>
    </owl:NamedIndividual>
    


    <!-- http://purl.obolibrary.org/obo/GAZ_00142137 -->

    <owl:NamedIndividual rdf:about="http://purl.obolibrary.org/obo/GAZ_00142137">
        <obo:RO_0001025 rdf:resource="http://purl.obolibrary.org/obo/GAZ_00009561"/>
        <obo:IAO_0000115>The SW reef of the Fakaofo Atoll, apparently unamed.</obo:IAO_0000115>
        <oboInOwl:hasOBONamespace>GAZ</oboInOwl:hasOBONamespace>
        <oboInOwl:id>GAZ:00142137</oboInOwl:id>
        <rdfs:label>South West Reef</rdfs:label>
    </owl:NamedIndividual>
    


    <!-- http://purl.obolibrary.org/obo/GAZ_00142138 -->

    <owl:NamedIndividual rdf:about="http://purl.obolibrary.org/obo/GAZ_00142138">
        <obo:RO_0001025 rdf:resource="http://purl.obolibrary.org/obo/GAZ_00142136"/>
        <obo:IAO_0000115>The SE reef of the Fakaofo Atoll.</obo:IAO_0000115>
        <oboInOwl:hasOBONamespace>GAZ</oboInOwl:hasOBONamespace>
        <oboInOwl:id>GAZ:00142138</oboInOwl:id>
        <rdfs:label>Kapiomotu</rdfs:label>
    </owl:NamedIndividual>
    


    <!-- http://purl.obolibrary.org/obo/GAZ_00142139 -->

    <owl:NamedIndividual rdf:about="http://purl.obolibrary.org/obo/GAZ_00142139">
        <obo:RO_0001025 rdf:resource="http://purl.obolibrary.org/obo/GAZ_02000337"/>
        <obo:IAO_0000115>The brackish central lagoon of the Swains Island atoll.</obo:IAO_0000115>
        <oboInOwl:hasOBONamespace>GAZ</oboInOwl:hasOBONamespace>
        <oboInOwl:id>GAZ:00142139</oboInOwl:id>
        <rdfs:label>Swains Island Lagoon</rdfs:label>
    </owl:NamedIndividual>
    


    <!-- http://purl.obolibrary.org/obo/GAZ_00142140 -->

    <owl:NamedIndividual rdf:about="http://purl.obolibrary.org/obo/GAZ_00142140">
        <obo:RO_0001025 rdf:resource="http://purl.obolibrary.org/obo/GAZ_00009562"/>
        <obo:IAO_0000115>The central lagoon of the Atafu Atoll.</obo:IAO_0000115>
        <oboInOwl:hasOBONamespace>GAZ</oboInOwl:hasOBONamespace>
        <oboInOwl:id>GAZ:00142140</oboInOwl:id>
        <rdfs:label>Atafu Lagoon</rdfs:label>
    </owl:NamedIndividual>
    


    <!-- http://purl.obolibrary.org/obo/GAZ_00142141 -->

    <owl:NamedIndividual rdf:about="http://purl.obolibrary.org/obo/GAZ_00142141">
        <obo:RO_0001025 rdf:resource="http://purl.obolibrary.org/obo/GAZ_00009561"/>
        <obo:IAO_0000115>The central lagoon of the Fakaofo Atoll.</obo:IAO_0000115>
        <oboInOwl:hasOBONamespace>GAZ</oboInOwl:hasOBONamespace>
        <oboInOwl:id>GAZ:00142141</oboInOwl:id>
        <rdfs:label>Fakaofo Lagoon</rdfs:label>
    </owl:NamedIndividual>
    


    <!-- http://purl.obolibrary.org/obo/GAZ_00142142 -->

    <owl:NamedIndividual rdf:about="http://purl.obolibrary.org/obo/GAZ_00142142">
        <obo:RO_0001025 rdf:resource="http://purl.obolibrary.org/obo/GAZ_00009560"/>
        <obo:IAO_0000115>The central lagoon of the Nukunonu Atoll.</obo:IAO_0000115>
        <oboInOwl:hasOBONamespace>GAZ</oboInOwl:hasOBONamespace>
        <oboInOwl:id>GAZ:00142142</oboInOwl:id>
        <rdfs:label>Nukunonu Lagoon</rdfs:label>
    </owl:NamedIndividual>
    


    <!-- http://purl.obolibrary.org/obo/GAZ_00142143 -->

    <owl:NamedIndividual rdf:about="http://purl.obolibrary.org/obo/GAZ_00142143">
        <obo:RO_0001025 rdf:resource="http://purl.obolibrary.org/obo/GAZ_00044923"/>
        <obo:IAO_0000115>The SE headland of Rose Island.</obo:IAO_0000115>
        <oboInOwl:hasOBONamespace>GAZ</oboInOwl:hasOBONamespace>
        <oboInOwl:id>GAZ:00142143</oboInOwl:id>
        <rdfs:label>Lucas Head</rdfs:label>
    </owl:NamedIndividual>
    


    <!-- http://purl.obolibrary.org/obo/GAZ_00142149 -->

    <owl:NamedIndividual rdf:about="http://purl.obolibrary.org/obo/GAZ_00142149">
        <obo:RO_0001025 rdf:resource="http://purl.obolibrary.org/obo/GAZ_00017420"/>
        <obo:IAO_0000115>The SE point of Enderby Island.</obo:IAO_0000115>
        <oboInOwl:hasOBONamespace>GAZ</oboInOwl:hasOBONamespace>
        <oboInOwl:id>GAZ:00142149</oboInOwl:id>
        <rdfs:label>Pebble Point</rdfs:label>
    </owl:NamedIndividual>
    


    <!-- http://purl.obolibrary.org/obo/GAZ_00142150 -->

    <owl:NamedIndividual rdf:about="http://purl.obolibrary.org/obo/GAZ_00142150">
        <obo:RO_0001025 rdf:resource="http://purl.obolibrary.org/obo/GAZ_00017420"/>
        <obo:IAO_0000115>A small lake on the S of Enderby Island.</obo:IAO_0000115>
        <oboInOwl:hasOBONamespace>GAZ</oboInOwl:hasOBONamespace>
        <oboInOwl:id>GAZ:00142150</oboInOwl:id>
        <rdfs:label>Teal Lake</rdfs:label>
    </owl:NamedIndividual>
    


    <!-- http://purl.obolibrary.org/obo/GAZ_00142151 -->

    <owl:NamedIndividual rdf:about="http://purl.obolibrary.org/obo/GAZ_00142151">
        <obo:RO_0001025 rdf:resource="http://purl.obolibrary.org/obo/GAZ_00017420"/>
        <obo:IAO_0000115>An E point of Enderby Island.</obo:IAO_0000115>
        <oboInOwl:hasOBONamespace>GAZ</oboInOwl:hasOBONamespace>
        <oboInOwl:id>GAZ:00142151</oboInOwl:id>
        <rdfs:label>Gargoyle Point</rdfs:label>
    </owl:NamedIndividual>
    


    <!-- http://purl.obolibrary.org/obo/GAZ_00142152 -->

    <owl:NamedIndividual rdf:about="http://purl.obolibrary.org/obo/GAZ_00142152">
        <obo:RO_0001025 rdf:resource="http://purl.obolibrary.org/obo/GAZ_00017420"/>
        <obo:IAO_0000115>The most S point of Enderby Island.</obo:IAO_0000115>
        <oboInOwl:hasOBONamespace>GAZ</oboInOwl:hasOBONamespace>
        <oboInOwl:id>GAZ:00142152</oboInOwl:id>
        <rdfs:label>Butterfield Point</rdfs:label>
    </owl:NamedIndividual>
    


    <!-- http://purl.obolibrary.org/obo/GAZ_00142153 -->

    <owl:NamedIndividual rdf:about="http://purl.obolibrary.org/obo/GAZ_00142153">
        <obo:RO_0001025 rdf:resource="http://purl.obolibrary.org/obo/GAZ_00017420"/>
        <obo:IAO_0000115>An E cape of Enderby Island.</obo:IAO_0000115>
        <oboInOwl:hasOBONamespace>GAZ</oboInOwl:hasOBONamespace>
        <oboInOwl:id>GAZ:00142153</oboInOwl:id>
        <rdfs:label>North East Cape</rdfs:label>
    </owl:NamedIndividual>
    


    <!-- http://purl.obolibrary.org/obo/GAZ_00142154 -->

    <owl:NamedIndividual rdf:about="http://purl.obolibrary.org/obo/GAZ_00142154">
        <obo:RO_0001025 rdf:resource="http://purl.obolibrary.org/obo/GAZ_00017420"/>
        <obo:IAO_0000115>The W point of Enderby Island.</obo:IAO_0000115>
        <oboInOwl:hasOBONamespace>GAZ</oboInOwl:hasOBONamespace>
        <oboInOwl:id>GAZ:00142154</oboInOwl:id>
        <rdfs:label>Rapoka Point</rdfs:label>
    </owl:NamedIndividual>
    


    <!-- http://purl.obolibrary.org/obo/GAZ_00142155 -->

    <owl:NamedIndividual rdf:about="http://purl.obolibrary.org/obo/GAZ_00142155">
        <rdf:type rdf:resource="http://purl.obolibrary.org/obo/ENVO_00000305"/>
        <obo:RO_0001025 rdf:resource="http://purl.obolibrary.org/obo/GAZ_00017417"/>
        <obo:IAO_0000115>A SE cape of Adams Island.</obo:IAO_0000115>
        <oboInOwl:hasOBONamespace>GAZ</oboInOwl:hasOBONamespace>
        <oboInOwl:id>GAZ:00142155</oboInOwl:id>
        <rdfs:label>Cape Thompson</rdfs:label>
    </owl:NamedIndividual>
    


    <!-- http://purl.obolibrary.org/obo/GAZ_00142156 -->

    <owl:NamedIndividual rdf:about="http://purl.obolibrary.org/obo/GAZ_00142156">
        <obo:RO_0001025 rdf:resource="http://purl.obolibrary.org/obo/GAZ_00017417"/>
        <obo:IAO_0000115>The E headland of Adams Island.</obo:IAO_0000115>
        <oboInOwl:hasOBONamespace>GAZ</oboInOwl:hasOBONamespace>
        <oboInOwl:id>GAZ:00142156</oboInOwl:id>
        <rdfs:label>Gilroy Head</rdfs:label>
    </owl:NamedIndividual>
    


    <!-- http://purl.obolibrary.org/obo/GAZ_00142157 -->

    <owl:NamedIndividual rdf:about="http://purl.obolibrary.org/obo/GAZ_00142157">
        <rdf:type rdf:resource="http://purl.obolibrary.org/obo/ENVO_00000167"/>
        <obo:RO_0001025 rdf:resource="http://purl.obolibrary.org/obo/GAZ_00017417"/>
        <obo:IAO_0000115>A SE point of Adams Island.</obo:IAO_0000115>
        <oboInOwl:hasOBONamespace>GAZ</oboInOwl:hasOBONamespace>
        <oboInOwl:id>GAZ:00142157</oboInOwl:id>
        <rdfs:label>Castle Point</rdfs:label>
    </owl:NamedIndividual>
    


    <!-- http://purl.obolibrary.org/obo/GAZ_00142158 -->

    <owl:NamedIndividual rdf:about="http://purl.obolibrary.org/obo/GAZ_00142158">
        <obo:RO_0001025 rdf:resource="http://purl.obolibrary.org/obo/GAZ_00017417"/>
        <obo:IAO_0000115>A cirque lake dammed by a rock threshold.</obo:IAO_0000115>
        <oboInOwl:hasOBONamespace>GAZ</oboInOwl:hasOBONamespace>
        <oboInOwl:id>GAZ:00142158</oboInOwl:id>
        <rdfs:label>Lake Turbott</rdfs:label>
    </owl:NamedIndividual>
    


    <!-- http://purl.obolibrary.org/obo/GAZ_00142159 -->

    <owl:NamedIndividual rdf:about="http://purl.obolibrary.org/obo/GAZ_00142159">
        <obo:RO_0001025 rdf:resource="http://purl.obolibrary.org/obo/GAZ_00017417"/>
        <obo:IAO_0000115>The S cape of Adams Island.</obo:IAO_0000115>
        <oboInOwl:hasOBONamespace>GAZ</oboInOwl:hasOBONamespace>
        <oboInOwl:id>GAZ:00142159</oboInOwl:id>
        <rdfs:label>South Cape</rdfs:label>
    </owl:NamedIndividual>
    


    <!-- http://purl.obolibrary.org/obo/GAZ_00142160 -->

    <owl:NamedIndividual rdf:about="http://purl.obolibrary.org/obo/GAZ_00142160">
        <obo:RO_0001025 rdf:resource="http://purl.obolibrary.org/obo/GAZ_00017417"/>
        <obo:IAO_0000115>A W point of Adams Island.</obo:IAO_0000115>
        <oboInOwl:hasOBONamespace>GAZ</oboInOwl:hasOBONamespace>
        <oboInOwl:id>GAZ:00142160</oboInOwl:id>
        <rdfs:label>Logan Point</rdfs:label>
    </owl:NamedIndividual>
    


    <!-- http://purl.obolibrary.org/obo/GAZ_00142161 -->

    <owl:NamedIndividual rdf:about="http://purl.obolibrary.org/obo/GAZ_00142161">
        <rdf:type rdf:resource="http://purl.obolibrary.org/obo/ENVO_00000167"/>
        <obo:RO_0001025 rdf:resource="http://purl.obolibrary.org/obo/GAZ_00017417"/>
        <obo:IAO_0000115>A SW point of Adams Island.</obo:IAO_0000115>
        <oboInOwl:hasOBONamespace>GAZ</oboInOwl:hasOBONamespace>
        <oboInOwl:id>GAZ:00142161</oboInOwl:id>
        <rdfs:label>Astrolabe Point</rdfs:label>
    </owl:NamedIndividual>
    


    <!-- http://purl.obolibrary.org/obo/GAZ_00142162 -->

    <owl:NamedIndividual rdf:about="http://purl.obolibrary.org/obo/GAZ_00142162">
        <obo:RO_0001025 rdf:resource="http://purl.obolibrary.org/obo/GAZ_00017417"/>
        <obo:IAO_0000115>The W point of Adams Island.</obo:IAO_0000115>
        <oboInOwl:hasOBONamespace>GAZ</oboInOwl:hasOBONamespace>
        <oboInOwl:id>GAZ:00142162</oboInOwl:id>
        <rdfs:label>Embrasure Point</rdfs:label>
    </owl:NamedIndividual>
    


    <!-- http://purl.obolibrary.org/obo/GAZ_00142163 -->

    <owl:NamedIndividual rdf:about="http://purl.obolibrary.org/obo/GAZ_00142163">
        <obo:RO_0001025 rdf:resource="http://purl.obolibrary.org/obo/GAZ_00017417"/>
        <obo:IAO_0000115>The N point of Adams Island.</obo:IAO_0000115>
        <oboInOwl:hasOBONamespace>GAZ</oboInOwl:hasOBONamespace>
        <oboInOwl:id>GAZ:00142163</oboInOwl:id>
        <rdfs:label>Grafton Point</rdfs:label>
    </owl:NamedIndividual>
    


    <!-- http://purl.obolibrary.org/obo/GAZ_00142164 -->

    <owl:NamedIndividual rdf:about="http://purl.obolibrary.org/obo/GAZ_00142164">
        <rdf:type rdf:resource="http://purl.obolibrary.org/obo/ENVO_00000305"/>
        <obo:RO_0001025 rdf:resource="http://purl.obolibrary.org/obo/GAZ_00017418"/>
        <obo:IAO_0000115>A headland at the N entrance to Laurie Harbour.</obo:IAO_0000115>
        <oboInOwl:hasOBONamespace>GAZ</oboInOwl:hasOBONamespace>
        <oboInOwl:id>GAZ:00142164</oboInOwl:id>
        <rdfs:label>Beacon Point</rdfs:label>
    </owl:NamedIndividual>
    


    <!-- http://purl.obolibrary.org/obo/GAZ_00142165 -->

    <owl:NamedIndividual rdf:about="http://purl.obolibrary.org/obo/GAZ_00142165">
        <obo:RO_0001025 rdf:resource="http://purl.obolibrary.org/obo/GAZ_00007173"/>
        <obo:IAO_0000115>A rock NW of Bristow Point.</obo:IAO_0000115>
        <oboInOwl:hasOBONamespace>GAZ</oboInOwl:hasOBONamespace>
        <oboInOwl:id>GAZ:00142165</oboInOwl:id>
        <rdfs:label>Detached Rock</rdfs:label>
    </owl:NamedIndividual>
    


    <!-- http://purl.obolibrary.org/obo/GAZ_00142166 -->

    <owl:NamedIndividual rdf:about="http://purl.obolibrary.org/obo/GAZ_00142166">
        <obo:RO_0001025 rdf:resource="http://purl.obolibrary.org/obo/GAZ_00007173"/>
        <obo:IAO_0000115>A small rock off the W coast of Auckland Island.</obo:IAO_0000115>
        <oboInOwl:hasOBONamespace>GAZ</oboInOwl:hasOBONamespace>
        <oboInOwl:id>GAZ:00142166</oboInOwl:id>
        <rdfs:label>Beehive Rock</rdfs:label>
    </owl:NamedIndividual>
    


    <!-- http://purl.obolibrary.org/obo/GAZ_00142167 -->

    <owl:NamedIndividual rdf:about="http://purl.obolibrary.org/obo/GAZ_00142167">
        <obo:RO_0001025 rdf:resource="http://purl.obolibrary.org/obo/GAZ_00017418"/>
        <obo:IAO_0000115>The most N point of Auckland Island.</obo:IAO_0000115>
        <oboInOwl:hasOBONamespace>GAZ</oboInOwl:hasOBONamespace>
        <oboInOwl:id>GAZ:00142167</oboInOwl:id>
        <rdfs:label>North Point</rdfs:label>
    </owl:NamedIndividual>
    


    <!-- http://purl.obolibrary.org/obo/GAZ_00142168 -->

    <owl:NamedIndividual rdf:about="http://purl.obolibrary.org/obo/GAZ_00142168">
        <obo:RO_0001025 rdf:resource="http://purl.obolibrary.org/obo/GAZ_00017418"/>
        <obo:IAO_0000115>The SW point of Auckland Island.</obo:IAO_0000115>
        <oboInOwl:hasOBONamespace>GAZ</oboInOwl:hasOBONamespace>
        <oboInOwl:id>GAZ:00142168</oboInOwl:id>
        <rdfs:label>South West Cape</rdfs:label>
    </owl:NamedIndividual>
    


    <!-- http://purl.obolibrary.org/obo/GAZ_00142169 -->

    <owl:NamedIndividual rdf:about="http://purl.obolibrary.org/obo/GAZ_00142169">
        <obo:RO_0001025 rdf:resource="http://purl.obolibrary.org/obo/GAZ_00017418"/>
        <obo:IAO_0000115>A headland S of Terror Cove.</obo:IAO_0000115>
        <oboInOwl:hasOBONamespace>GAZ</oboInOwl:hasOBONamespace>
        <oboInOwl:id>GAZ:00142169</oboInOwl:id>
        <rdfs:label>Johnson Point</rdfs:label>
    </owl:NamedIndividual>
    


    <!-- http://purl.obolibrary.org/obo/GAZ_00142170 -->

    <owl:NamedIndividual rdf:about="http://purl.obolibrary.org/obo/GAZ_00142170">
        <rdf:type rdf:resource="http://purl.obolibrary.org/obo/ENVO_00000167"/>
        <obo:RO_0001025 rdf:resource="http://purl.obolibrary.org/obo/GAZ_00017418"/>
        <obo:IAO_0000115>A NE point of Auckland Island.</obo:IAO_0000115>
        <oboInOwl:hasOBONamespace>GAZ</oboInOwl:hasOBONamespace>
        <oboInOwl:id>GAZ:00142170</oboInOwl:id>
        <rdfs:label>Tucker Point</rdfs:label>
    </owl:NamedIndividual>
    


    <!-- http://purl.obolibrary.org/obo/GAZ_00142171 -->

    <owl:NamedIndividual rdf:about="http://purl.obolibrary.org/obo/GAZ_00142171">
        <rdf:type rdf:resource="http://purl.obolibrary.org/obo/ENVO_00000167"/>
        <obo:RO_0001025 rdf:resource="http://purl.obolibrary.org/obo/GAZ_00017418"/>
        <obo:IAO_0000115>A NE point of Auckland Island.</obo:IAO_0000115>
        <oboInOwl:hasOBONamespace>GAZ</oboInOwl:hasOBONamespace>
        <oboInOwl:id>GAZ:00142171</oboInOwl:id>
        <rdfs:label>Lindley Point</rdfs:label>
    </owl:NamedIndividual>
    


    <!-- http://purl.obolibrary.org/obo/GAZ_00142172 -->

    <owl:NamedIndividual rdf:about="http://purl.obolibrary.org/obo/GAZ_00142172">
        <rdf:type rdf:resource="http://purl.obolibrary.org/obo/ENVO_00000305"/>
        <obo:RO_0001025 rdf:resource="http://purl.obolibrary.org/obo/GAZ_00017418"/>
        <obo:IAO_0000115>A SW cape of Auckland Island.</obo:IAO_0000115>
        <oboInOwl:hasOBONamespace>GAZ</oboInOwl:hasOBONamespace>
        <oboInOwl:id>GAZ:00142172</oboInOwl:id>
        <rdfs:label>Bristow Point</rdfs:label>
    </owl:NamedIndividual>
    


    <!-- http://purl.obolibrary.org/obo/GAZ_00142173 -->

    <owl:NamedIndividual rdf:about="http://purl.obolibrary.org/obo/GAZ_00142173">
        <rdf:type rdf:resource="http://purl.obolibrary.org/obo/ENVO_00000167"/>
        <obo:RO_0001025 rdf:resource="http://purl.obolibrary.org/obo/GAZ_00017418"/>
        <obo:IAO_0000115>A NW point of Auckland Island.</obo:IAO_0000115>
        <oboInOwl:hasOBONamespace>GAZ</oboInOwl:hasOBONamespace>
        <oboInOwl:id>GAZ:00142173</oboInOwl:id>
        <rdfs:label>Black Head</rdfs:label>
    </owl:NamedIndividual>
    


    <!-- http://purl.obolibrary.org/obo/GAZ_00142174 -->

    <owl:NamedIndividual rdf:about="http://purl.obolibrary.org/obo/GAZ_00142174">
        <rdf:type rdf:resource="http://purl.obolibrary.org/obo/ENVO_00000305"/>
        <obo:RO_0001025 rdf:resource="http://purl.obolibrary.org/obo/GAZ_00017418"/>
        <obo:IAO_0000115>A SW cape of Auckland Island.</obo:IAO_0000115>
        <oboInOwl:hasOBONamespace>GAZ</oboInOwl:hasOBONamespace>
        <oboInOwl:id>GAZ:00142174</oboInOwl:id>
        <rdfs:label>Cape Lovitt</rdfs:label>
    </owl:NamedIndividual>
    


    <!-- http://purl.obolibrary.org/obo/GAZ_00142175 -->

    <owl:NamedIndividual rdf:about="http://purl.obolibrary.org/obo/GAZ_00142175">
        <obo:RO_0001025 rdf:resource="http://purl.obolibrary.org/obo/GAZ_00017418"/>
        <obo:IAO_0000115>A headland projecting from the S into Laurie Harbour.</obo:IAO_0000115>
        <oboInOwl:hasOBONamespace>GAZ</oboInOwl:hasOBONamespace>
        <oboInOwl:id>GAZ:00142175</oboInOwl:id>
        <rdfs:label>Williamson Point</rdfs:label>
    </owl:NamedIndividual>
    


    <!-- http://purl.obolibrary.org/obo/GAZ_00142176 -->

    <owl:NamedIndividual rdf:about="http://purl.obolibrary.org/obo/GAZ_00142176">
        <obo:RO_0001025 rdf:resource="http://purl.obolibrary.org/obo/GAZ_00017418"/>
        <obo:IAO_0000115>The NE point of Auckland Island.</obo:IAO_0000115>
        <oboInOwl:hasOBONamespace>GAZ</oboInOwl:hasOBONamespace>
        <oboInOwl:id>GAZ:00142176</oboInOwl:id>
        <rdfs:label>Crozier Point</rdfs:label>
    </owl:NamedIndividual>
    


    <!-- http://purl.obolibrary.org/obo/GAZ_00142177 -->

    <owl:NamedIndividual rdf:about="http://purl.obolibrary.org/obo/GAZ_00142177">
        <obo:RO_0001025 rdf:resource="http://purl.obolibrary.org/obo/GAZ_00017418"/>
        <obo:IAO_0000115>The NW cape of the Auckland Islands.</obo:IAO_0000115>
        <oboInOwl:hasOBONamespace>GAZ</oboInOwl:hasOBONamespace>
        <oboInOwl:id>GAZ:00142177</oboInOwl:id>
        <rdfs:label>North West Cape</rdfs:label>
    </owl:NamedIndividual>
    


    <!-- http://purl.obolibrary.org/obo/GAZ_00142178 -->

    <owl:NamedIndividual rdf:about="http://purl.obolibrary.org/obo/GAZ_00142178">
        <obo:RO_0001025 rdf:resource="http://purl.obolibrary.org/obo/GAZ_00017418"/>
        <obo:IAO_0000115>An E point of Auckland Island.</obo:IAO_0000115>
        <oboInOwl:hasOBONamespace>GAZ</oboInOwl:hasOBONamespace>
        <oboInOwl:id>GAZ:00142178</oboInOwl:id>
        <rdfs:label>Kekeno Point</rdfs:label>
    </owl:NamedIndividual>
    


    <!-- http://purl.obolibrary.org/obo/GAZ_00142179 -->

    <owl:NamedIndividual rdf:about="http://purl.obolibrary.org/obo/GAZ_00142179">
        <obo:RO_0001025 rdf:resource="http://purl.obolibrary.org/obo/GAZ_00017418"/>
        <obo:IAO_0000115>A peninsula on the E of Auckland Island, connected to the rest of the island by an isthmus.</obo:IAO_0000115>
        <oboInOwl:hasOBONamespace>GAZ</oboInOwl:hasOBONamespace>
        <oboInOwl:id>GAZ:00142179</oboInOwl:id>
        <rdfs:label>Falla Peninsula</rdfs:label>
    </owl:NamedIndividual>
    


    <!-- http://purl.obolibrary.org/obo/GAZ_00142180 -->

    <owl:NamedIndividual rdf:about="http://purl.obolibrary.org/obo/GAZ_00142180">
        <obo:RO_0001025 rdf:resource="http://purl.obolibrary.org/obo/GAZ_00017418"/>
        <obo:IAO_0000115>A headland jutting from the S into Waterfall Inlet.</obo:IAO_0000115>
        <oboInOwl:hasOBONamespace>GAZ</oboInOwl:hasOBONamespace>
        <oboInOwl:id>GAZ:00142180</oboInOwl:id>
        <rdfs:label>Shelter Point</rdfs:label>
    </owl:NamedIndividual>
    


    <!-- http://purl.obolibrary.org/obo/GAZ_00142181 -->

    <owl:NamedIndividual rdf:about="http://purl.obolibrary.org/obo/GAZ_00142181">
        <obo:RO_0001025 rdf:resource="http://purl.obolibrary.org/obo/GAZ_00017418"/>
        <obo:IAO_0000115>An E point of Auckland Island.</obo:IAO_0000115>
        <oboInOwl:hasOBONamespace>GAZ</oboInOwl:hasOBONamespace>
        <oboInOwl:id>GAZ:00142181</oboInOwl:id>
        <rdfs:label>Cape Bennett</rdfs:label>
    </owl:NamedIndividual>
    


    <!-- http://purl.obolibrary.org/obo/GAZ_00142182 -->

    <owl:NamedIndividual rdf:about="http://purl.obolibrary.org/obo/GAZ_00142182">
        <obo:RO_0001025 rdf:resource="http://purl.obolibrary.org/obo/GAZ_00017418"/>
        <obo:IAO_0000115>An E point of Auckland Island.</obo:IAO_0000115>
        <oboInOwl:hasOBONamespace>GAZ</oboInOwl:hasOBONamespace>
        <oboInOwl:id>GAZ:00142182</oboInOwl:id>
        <rdfs:label>Signboard Point</rdfs:label>
    </owl:NamedIndividual>
    


    <!-- http://purl.obolibrary.org/obo/GAZ_00142183 -->

    <owl:NamedIndividual rdf:about="http://purl.obolibrary.org/obo/GAZ_00142183">
        <rdf:type rdf:resource="http://purl.obolibrary.org/obo/ENVO_00000305"/>
        <obo:RO_0001025 rdf:resource="http://purl.obolibrary.org/obo/GAZ_00017418"/>
        <obo:IAO_0000115>A headland to the SW of Tongue Bay, projecting into Carnley Harbour.</obo:IAO_0000115>
        <oboInOwl:hasOBONamespace>GAZ</oboInOwl:hasOBONamespace>
        <oboInOwl:id>GAZ:00142183</oboInOwl:id>
        <rdfs:label>Emergency Point</rdfs:label>
    </owl:NamedIndividual>
    


    <!-- http://purl.obolibrary.org/obo/GAZ_00142184 -->

    <owl:NamedIndividual rdf:about="http://purl.obolibrary.org/obo/GAZ_00142184">
        <obo:RO_0001025 rdf:resource="http://purl.obolibrary.org/obo/GAZ_00017418"/>
        <obo:IAO_0000115>The SE point of Auckland Islan.</obo:IAO_0000115>
        <oboInOwl:hasOBONamespace>GAZ</oboInOwl:hasOBONamespace>
        <oboInOwl:id>GAZ:00142184</oboInOwl:id>
        <rdfs:label>Cape Farr</rdfs:label>
    </owl:NamedIndividual>
    


    <!-- http://purl.obolibrary.org/obo/GAZ_00142185 -->

    <owl:NamedIndividual rdf:about="http://purl.obolibrary.org/obo/GAZ_00142185">
        <rdf:type rdf:resource="http://purl.obolibrary.org/obo/ENVO_00000305"/>
        <obo:RO_0001025 rdf:resource="http://purl.obolibrary.org/obo/GAZ_00017418"/>
        <obo:IAO_0000115>A SW headland of Auckland Island.</obo:IAO_0000115>
        <oboInOwl:hasOBONamespace>GAZ</oboInOwl:hasOBONamespace>
        <oboInOwl:id>GAZ:00142185</oboInOwl:id>
        <rdfs:label>Perpendicular Head</rdfs:label>
    </owl:NamedIndividual>
    


    <!-- http://purl.obolibrary.org/obo/GAZ_00142186 -->

    <owl:NamedIndividual rdf:about="http://purl.obolibrary.org/obo/GAZ_00142186">
        <obo:RO_0001025 rdf:resource="http://purl.obolibrary.org/obo/GAZ_00017418"/>
        <obo:IAO_0000115>A headland projecting into the S end of North Arm from the E.</obo:IAO_0000115>
        <oboInOwl:hasOBONamespace>GAZ</oboInOwl:hasOBONamespace>
        <oboInOwl:id>GAZ:00142186</oboInOwl:id>
        <rdfs:label>Raynal Point</rdfs:label>
    </owl:NamedIndividual>
    


    <!-- http://purl.obolibrary.org/obo/GAZ_00142187 -->

    <owl:NamedIndividual rdf:about="http://purl.obolibrary.org/obo/GAZ_00142187">
        <obo:RO_0001025 rdf:resource="http://purl.obolibrary.org/obo/GAZ_00017418"/>
        <obo:IAO_0000115>A peninsula, connected to Auckland Island by an isthmus, projecting into Carnley Harbour.</obo:IAO_0000115>
        <oboInOwl:hasOBONamespace>GAZ</oboInOwl:hasOBONamespace>
        <oboInOwl:id>GAZ:00142187</oboInOwl:id>
        <rdfs:label>Musgrave Peninsula</rdfs:label>
    </owl:NamedIndividual>
    


    <!-- http://purl.obolibrary.org/obo/GAZ_00142188 -->

    <owl:NamedIndividual rdf:about="http://purl.obolibrary.org/obo/GAZ_00142188">
        <obo:RO_0001025 rdf:resource="http://purl.obolibrary.org/obo/GAZ_00142187"/>
        <obo:IAO_0000115>The S point of the Musgrave Peninsula.</obo:IAO_0000115>
        <oboInOwl:hasOBONamespace>GAZ</oboInOwl:hasOBONamespace>
        <oboInOwl:id>GAZ:00142188</oboInOwl:id>
        <rdfs:label>Flagstaff Point</rdfs:label>
    </owl:NamedIndividual>
    


    <!-- http://purl.obolibrary.org/obo/GAZ_00142189 -->

    <owl:NamedIndividual rdf:about="http://purl.obolibrary.org/obo/GAZ_00142189">
        <obo:RO_0001025 rdf:resource="http://purl.obolibrary.org/obo/GAZ_00142187"/>
        <obo:IAO_0000115>The N point of the Musgrave Peninsula.</obo:IAO_0000115>
        <oboInOwl:hasOBONamespace>GAZ</oboInOwl:hasOBONamespace>
        <oboInOwl:id>GAZ:00142189</oboInOwl:id>
        <rdfs:label>Granite Point</rdfs:label>
    </owl:NamedIndividual>
    


    <!-- http://purl.obolibrary.org/obo/GAZ_00142190 -->

    <owl:NamedIndividual rdf:about="http://purl.obolibrary.org/obo/GAZ_00142190">
        <obo:RO_0001025 rdf:resource="http://purl.obolibrary.org/obo/GAZ_00017418"/>
        <obo:IAO_0000115>A peninsula forming the W side of North Arm.</obo:IAO_0000115>
        <oboInOwl:hasOBONamespace>GAZ</oboInOwl:hasOBONamespace>
        <oboInOwl:id>GAZ:00142190</oboInOwl:id>
        <rdfs:label>Circular Head</rdfs:label>
    </owl:NamedIndividual>
    


    <!-- http://purl.obolibrary.org/obo/GAZ_00142191 -->

    <owl:NamedIndividual rdf:about="http://purl.obolibrary.org/obo/GAZ_00142191">
        <obo:RO_0001025 rdf:resource="http://purl.obolibrary.org/obo/GAZ_00017418"/>
        <obo:IAO_0000115>A peninsula between Coleridge Bay (to the S) and Musgrave Harbour (to the N).</obo:IAO_0000115>
        <oboInOwl:hasOBONamespace>GAZ</oboInOwl:hasOBONamespace>
        <oboInOwl:id>GAZ:00142191</oboInOwl:id>
        <rdfs:label>McClure Head</rdfs:label>
    </owl:NamedIndividual>
    


    <!-- http://purl.obolibrary.org/obo/GAZ_00142192 -->

    <owl:NamedIndividual rdf:about="http://purl.obolibrary.org/obo/GAZ_00142192">
        <obo:RO_0001025 rdf:resource="http://purl.obolibrary.org/obo/GAZ_00017418"/>
        <obo:IAO_0000115>A shallow point on the NE coast of North Arm.</obo:IAO_0000115>
        <oboInOwl:hasOBONamespace>GAZ</oboInOwl:hasOBONamespace>
        <oboInOwl:id>GAZ:00142192</oboInOwl:id>
        <rdfs:label>Round Point</rdfs:label>
    </owl:NamedIndividual>
    


    <!-- http://purl.obolibrary.org/obo/GAZ_00142193 -->

    <owl:NamedIndividual rdf:about="http://purl.obolibrary.org/obo/GAZ_00142193">
        <rdf:type rdf:resource="http://purl.obolibrary.org/obo/ENVO_00000305"/>
        <obo:RO_0001025 rdf:resource="http://purl.obolibrary.org/obo/GAZ_00017418"/>
        <obo:IAO_0000115>A headland to the NE of Camp Cove.</obo:IAO_0000115>
        <oboInOwl:hasOBONamespace>GAZ</oboInOwl:hasOBONamespace>
        <oboInOwl:id>GAZ:00142193</oboInOwl:id>
        <rdfs:label>Anjou Point</rdfs:label>
    </owl:NamedIndividual>
    


    <!-- http://purl.obolibrary.org/obo/GAZ_00142194 -->

    <owl:NamedIndividual rdf:about="http://purl.obolibrary.org/obo/GAZ_00142194">
        <rdf:type rdf:resource="http://purl.obolibrary.org/obo/ENVO_00000305"/>
        <obo:RO_0001025 rdf:resource="http://purl.obolibrary.org/obo/GAZ_00017418"/>
        <obo:IAO_0000115>A headland at the E end of Victoria Passage, N of Monumental Island.</obo:IAO_0000115>
        <oboInOwl:hasOBONamespace>GAZ</oboInOwl:hasOBONamespace>
        <oboInOwl:id>GAZ:00142194</oboInOwl:id>
        <rdfs:label>Breaksea Point</rdfs:label>
    </owl:NamedIndividual>
    


    <!-- http://purl.obolibrary.org/obo/GAZ_00142195 -->

    <owl:NamedIndividual rdf:about="http://purl.obolibrary.org/obo/GAZ_00142195">
        <obo:RO_0001025 rdf:resource="http://purl.obolibrary.org/obo/GAZ_00017418"/>
        <obo:IAO_0000115>A cirque lake W of Coleridge Bay.</obo:IAO_0000115>
        <oboInOwl:hasOBONamespace>GAZ</oboInOwl:hasOBONamespace>
        <oboInOwl:id>GAZ:00142195</oboInOwl:id>
        <rdfs:label>Lake Speight</rdfs:label>
    </owl:NamedIndividual>
    


    <!-- http://purl.obolibrary.org/obo/GAZ_00142196 -->

    <owl:NamedIndividual rdf:about="http://purl.obolibrary.org/obo/GAZ_00142196">
        <obo:RO_0001025 rdf:resource="http://purl.obolibrary.org/obo/GAZ_00017418"/>
        <obo:IAO_0000115>A moraine dammed lake in a glacial valley.</obo:IAO_0000115>
        <oboInOwl:hasOBONamespace>GAZ</oboInOwl:hasOBONamespace>
        <oboInOwl:id>GAZ:00142196</oboInOwl:id>
        <rdfs:label>Lake Hinemoa</rdfs:label>
    </owl:NamedIndividual>
    


    <!-- http://purl.obolibrary.org/obo/GAZ_00142197 -->

    <owl:NamedIndividual rdf:about="http://purl.obolibrary.org/obo/GAZ_00142197">
        <obo:RO_0001025 rdf:resource="http://purl.obolibrary.org/obo/GAZ_00017418"/>
        <obo:IAO_0000115>A moraine dammed lake in a glacial valley.</obo:IAO_0000115>
        <oboInOwl:hasOBONamespace>GAZ</oboInOwl:hasOBONamespace>
        <oboInOwl:id>GAZ:00142197</oboInOwl:id>
        <rdfs:label>Lake Tutanekai</rdfs:label>
    </owl:NamedIndividual>
    


    <!-- http://purl.obolibrary.org/obo/GAZ_00142198 -->

    <owl:NamedIndividual rdf:about="http://purl.obolibrary.org/obo/GAZ_00142198">
        <obo:RO_0001025 rdf:resource="http://purl.obolibrary.org/obo/GAZ_00017418"/>
        <obo:IAO_0000115>A headland SW of Lindley Point and NE of Johnson Point.</obo:IAO_0000115>
        <oboInOwl:hasOBONamespace>GAZ</oboInOwl:hasOBONamespace>
        <oboInOwl:id>GAZ:00142198</oboInOwl:id>
        <rdfs:label>Dea&apos;s Head</rdfs:label>
    </owl:NamedIndividual>
    


    <!-- http://purl.obolibrary.org/obo/GAZ_00142199 -->

    <owl:NamedIndividual rdf:about="http://purl.obolibrary.org/obo/GAZ_00142199">
        <obo:RO_0001025 rdf:resource="http://purl.obolibrary.org/obo/GAZ_00017418"/>
        <obo:IAO_0000115>A headland projecting S into Hanfield Inlet.</obo:IAO_0000115>
        <oboInOwl:hasOBONamespace>GAZ</oboInOwl:hasOBONamespace>
        <oboInOwl:id>GAZ:00142199</oboInOwl:id>
        <rdfs:label>Middle Head</rdfs:label>
    </owl:NamedIndividual>
    


    <!-- http://purl.obolibrary.org/obo/GAZ_00142225 -->

    <owl:NamedIndividual rdf:about="http://purl.obolibrary.org/obo/GAZ_00142225">
        <obo:RO_0001025 rdf:resource="http://purl.obolibrary.org/obo/GAZ_00017420"/>
        <obo:IAO_0000115>A stream on Enderby Island.</obo:IAO_0000115>
        <oboInOwl:hasOBONamespace>GAZ</oboInOwl:hasOBONamespace>
        <oboInOwl:id>GAZ:00142225</oboInOwl:id>
        <rdfs:label>Stella Creek</rdfs:label>
    </owl:NamedIndividual>
    


    <!-- http://purl.obolibrary.org/obo/GAZ_00142226 -->

    <owl:NamedIndividual rdf:about="http://purl.obolibrary.org/obo/GAZ_00142226">
        <obo:RO_0001025 rdf:resource="http://purl.obolibrary.org/obo/GAZ_00017420"/>
        <obo:IAO_0000115>A stream on Enderby Island, in the SE.</obo:IAO_0000115>
        <oboInOwl:hasOBONamespace>GAZ</oboInOwl:hasOBONamespace>
        <oboInOwl:id>GAZ:00142226</oboInOwl:id>
        <rdfs:label>Hoiho Creek</rdfs:label>
    </owl:NamedIndividual>
    


    <!-- http://purl.obolibrary.org/obo/GAZ_00142227 -->

    <owl:NamedIndividual rdf:about="http://purl.obolibrary.org/obo/GAZ_00142227">
        <obo:RO_0001025 rdf:resource="http://purl.obolibrary.org/obo/GAZ_00017420"/>
        <obo:IAO_0000115>A stream on Enderby Island, in the NE.</obo:IAO_0000115>
        <oboInOwl:hasOBONamespace>GAZ</oboInOwl:hasOBONamespace>
        <oboInOwl:id>GAZ:00142227</oboInOwl:id>
        <rdfs:label>Spat Creek</rdfs:label>
    </owl:NamedIndividual>
    


    <!-- http://purl.obolibrary.org/obo/GAZ_00142228 -->

    <owl:NamedIndividual rdf:about="http://purl.obolibrary.org/obo/GAZ_00142228">
        <obo:RO_0001025 rdf:resource="http://purl.obolibrary.org/obo/GAZ_00017418"/>
        <obo:IAO_0000115>A stream on Auckland Island draining into the head of Laurie Harbour.</obo:IAO_0000115>
        <oboInOwl:hasOBONamespace>GAZ</oboInOwl:hasOBONamespace>
        <oboInOwl:id>GAZ:00142228</oboInOwl:id>
        <rdfs:label>Grey Dick Creek</rdfs:label>
    </owl:NamedIndividual>
    


    <!-- http://purl.obolibrary.org/obo/GAZ_00142229 -->

    <owl:NamedIndividual rdf:about="http://purl.obolibrary.org/obo/GAZ_00142229">
        <obo:RO_0001025 rdf:resource="http://purl.obolibrary.org/obo/GAZ_00017418"/>
        <obo:IAO_0000115>A stream on Auckland Island draining into the S of Laurie Bay.</obo:IAO_0000115>
        <oboInOwl:hasOBONamespace>GAZ</oboInOwl:hasOBONamespace>
        <oboInOwl:id>GAZ:00142229</oboInOwl:id>
        <rdfs:label>Sealers Creek</rdfs:label>
    </owl:NamedIndividual>
    


    <!-- http://purl.obolibrary.org/obo/GAZ_00142230 -->

    <owl:NamedIndividual rdf:about="http://purl.obolibrary.org/obo/GAZ_00142230">
        <rdf:type rdf:resource="http://purl.obolibrary.org/obo/ENVO_00000305"/>
        <obo:RO_0001025 rdf:resource="http://purl.obolibrary.org/obo/GAZ_00044991"/>
        <obo:IAO_0000115>A headland on the E coast of North East Island.</obo:IAO_0000115>
        <oboInOwl:hasOBONamespace>GAZ</oboInOwl:hasOBONamespace>
        <oboInOwl:id>GAZ:00142230</oboInOwl:id>
        <rdfs:label>Skua Rock</rdfs:label>
    </owl:NamedIndividual>
    


    <!-- http://purl.obolibrary.org/obo/GAZ_00142231 -->

    <owl:NamedIndividual rdf:about="http://purl.obolibrary.org/obo/GAZ_00142231">
        <obo:RO_0001025 rdf:resource="http://purl.obolibrary.org/obo/GAZ_00007143"/>
        <obo:IAO_0000115>The SW point of Raoul Island.</obo:IAO_0000115>
        <oboInOwl:hasOBONamespace>GAZ</oboInOwl:hasOBONamespace>
        <oboInOwl:id>GAZ:00142231</oboInOwl:id>
        <rdfs:label>Smith Bluff</rdfs:label>
    </owl:NamedIndividual>
    


    <!-- http://purl.obolibrary.org/obo/GAZ_00142232 -->

    <owl:NamedIndividual rdf:about="http://purl.obolibrary.org/obo/GAZ_00142232">
        <obo:RO_0001025 rdf:resource="http://purl.obolibrary.org/obo/GAZ_00044991"/>
        <obo:IAO_0000115>A peninsula on the E coast of North East Island, S of Skua Point.</obo:IAO_0000115>
        <oboInOwl:hasOBONamespace>GAZ</oboInOwl:hasOBONamespace>
        <oboInOwl:id>GAZ:00142232</oboInOwl:id>
        <rdfs:label>Seal Point</rdfs:label>
    </owl:NamedIndividual>
    


    <!-- http://purl.obolibrary.org/obo/GAZ_00142237 -->

    <owl:NamedIndividual rdf:about="http://purl.obolibrary.org/obo/GAZ_00142237">
        <obo:RO_0001025 rdf:resource="http://purl.obolibrary.org/obo/GAZ_00007143"/>
        <obo:IAO_0000115>The S point of Raoul Island.</obo:IAO_0000115>
        <oboInOwl:hasOBONamespace>GAZ</oboInOwl:hasOBONamespace>
        <oboInOwl:id>GAZ:00142237</oboInOwl:id>
        <rdfs:label>D&apos;Arcy Point</rdfs:label>
    </owl:NamedIndividual>
    


    <!-- http://purl.obolibrary.org/obo/GAZ_00142240 -->

    <owl:NamedIndividual rdf:about="http://purl.obolibrary.org/obo/GAZ_00142240">
        <obo:RO_0001025 rdf:resource="http://purl.obolibrary.org/obo/GAZ_00007143"/>
        <obo:IAO_0000115>A plain.</obo:IAO_0000115>
        <oboInOwl:hasOBONamespace>GAZ</oboInOwl:hasOBONamespace>
        <oboInOwl:id>GAZ:00142240</oboInOwl:id>
        <rdfs:label>Pumice Flats</rdfs:label>
    </owl:NamedIndividual>
    


    <!-- http://purl.obolibrary.org/obo/GAZ_00142241 -->

    <owl:NamedIndividual rdf:about="http://purl.obolibrary.org/obo/GAZ_00142241">
        <obo:RO_0001025 rdf:resource="http://purl.obolibrary.org/obo/GAZ_00142240"/>
        <obo:IAO_0000115>A stream flowing into Green Lake.</obo:IAO_0000115>
        <oboInOwl:hasOBONamespace>GAZ</oboInOwl:hasOBONamespace>
        <oboInOwl:id>GAZ:00142241</oboInOwl:id>
        <rdfs:label>Crater Creek</rdfs:label>
    </owl:NamedIndividual>
    


    <!-- http://purl.obolibrary.org/obo/GAZ_00142242 -->

    <owl:NamedIndividual rdf:about="http://purl.obolibrary.org/obo/GAZ_00142242">
        <obo:RO_0001025 rdf:resource="http://purl.obolibrary.org/obo/GAZ_00007143"/>
        <obo:IAO_0000115>A valley in the SW of Raoul Island.</obo:IAO_0000115>
        <oboInOwl:hasOBONamespace>GAZ</oboInOwl:hasOBONamespace>
        <oboInOwl:id>GAZ:00142242</oboInOwl:id>
        <rdfs:label>Sunshine Valley</rdfs:label>
    </owl:NamedIndividual>
    


    <!-- http://purl.obolibrary.org/obo/GAZ_00142243 -->

    <owl:NamedIndividual rdf:about="http://purl.obolibrary.org/obo/GAZ_00142243">
        <obo:RO_0001025 rdf:resource="http://purl.obolibrary.org/obo/GAZ_00007143"/>
        <obo:IAO_0000115>The E point of Raoul Island.</obo:IAO_0000115>
        <oboInOwl:hasOBONamespace>GAZ</oboInOwl:hasOBONamespace>
        <oboInOwl:id>GAZ:00142243</oboInOwl:id>
        <rdfs:label>Wilson Point</rdfs:label>
    </owl:NamedIndividual>
    


    <!-- http://purl.obolibrary.org/obo/GAZ_00142244 -->

    <owl:NamedIndividual rdf:about="http://purl.obolibrary.org/obo/GAZ_00142244">
        <rdf:type rdf:resource="http://purl.obolibrary.org/obo/ENVO_00000167"/>
        <obo:RO_0001025 rdf:resource="http://purl.obolibrary.org/obo/GAZ_00007143"/>
        <obo:IAO_0000115>A SE point of Raoul Island.</obo:IAO_0000115>
        <oboInOwl:hasOBONamespace>GAZ</oboInOwl:hasOBONamespace>
        <oboInOwl:id>GAZ:00142244</oboInOwl:id>
        <rdfs:label>Te Konui Point</rdfs:label>
    </owl:NamedIndividual>
    


    <!-- http://purl.obolibrary.org/obo/GAZ_00142245 -->

    <owl:NamedIndividual rdf:about="http://purl.obolibrary.org/obo/GAZ_00142245">
        <obo:RO_0001025 rdf:resource="http://purl.obolibrary.org/obo/GAZ_00007143"/>
        <obo:IAO_0000115>A S point of Raoul Island, between Wilson Point and Te Konui Point.</obo:IAO_0000115>
        <oboInOwl:hasOBONamespace>GAZ</oboInOwl:hasOBONamespace>
        <oboInOwl:id>GAZ:00142245</oboInOwl:id>
        <rdfs:label>Nash Point</rdfs:label>
    </owl:NamedIndividual>
    


    <!-- http://purl.obolibrary.org/obo/GAZ_00142246 -->

    <owl:NamedIndividual rdf:about="http://purl.obolibrary.org/obo/GAZ_00142246">
        <rdf:type rdf:resource="http://purl.obolibrary.org/obo/ENVO_00000167"/>
        <obo:RO_0001025 rdf:resource="http://purl.obolibrary.org/obo/GAZ_00007143"/>
        <obo:IAO_0000115>A SE point of Raoul Island.</obo:IAO_0000115>
        <oboInOwl:hasOBONamespace>GAZ</oboInOwl:hasOBONamespace>
        <oboInOwl:id>GAZ:00142246</oboInOwl:id>
        <rdfs:label>Lava Point</rdfs:label>
    </owl:NamedIndividual>
    


    <!-- http://purl.obolibrary.org/obo/GAZ_00142247 -->

    <owl:NamedIndividual rdf:about="http://purl.obolibrary.org/obo/GAZ_00142247">
        <obo:RO_0001025 rdf:resource="http://purl.obolibrary.org/obo/GAZ_00007143"/>
        <obo:IAO_0000115>An E point of Raoul Island.</obo:IAO_0000115>
        <oboInOwl:hasOBONamespace>GAZ</oboInOwl:hasOBONamespace>
        <oboInOwl:id>GAZ:00142247</oboInOwl:id>
        <rdfs:label>Rayner Point</rdfs:label>
    </owl:NamedIndividual>
    


    <!-- http://purl.obolibrary.org/obo/GAZ_00142248 -->

    <owl:NamedIndividual rdf:about="http://purl.obolibrary.org/obo/GAZ_00142248">
        <obo:RO_0001025 rdf:resource="http://purl.obolibrary.org/obo/GAZ_00007143"/>
        <obo:IAO_0000115>The NW point of Raoul Island.</obo:IAO_0000115>
        <oboInOwl:hasOBONamespace>GAZ</oboInOwl:hasOBONamespace>
        <oboInOwl:id>GAZ:00142248</oboInOwl:id>
        <rdfs:label>Hutchison Bluff</rdfs:label>
    </owl:NamedIndividual>
    


    <!-- http://purl.obolibrary.org/obo/GAZ_00142251 -->

    <owl:NamedIndividual rdf:about="http://purl.obolibrary.org/obo/GAZ_00142251">
        <obo:RO_0001025 rdf:resource="http://purl.obolibrary.org/obo/GAZ_00007143"/>
        <obo:IAO_0000115>A New Zealand meteorological station located above the cliffs of Fleetwood Bluff.</obo:IAO_0000115>
        <oboInOwl:hasOBONamespace>GAZ</oboInOwl:hasOBONamespace>
        <oboInOwl:id>GAZ:00142251</oboInOwl:id>
        <rdfs:label>Raoul Island Station</rdfs:label>
    </owl:NamedIndividual>
    


    <!-- http://purl.obolibrary.org/obo/GAZ_00142485 -->

    <owl:NamedIndividual rdf:about="http://purl.obolibrary.org/obo/GAZ_00142485">
        <obo:RO_0001025 rdf:resource="http://purl.obolibrary.org/obo/GAZ_00007175"/>
        <obo:IAO_0000115>A small island off the NW of Campbell Island, SW of Courrejolles Point.</obo:IAO_0000115>
        <oboInOwl:hasOBONamespace>GAZ</oboInOwl:hasOBONamespace>
        <oboInOwl:id>GAZ:00142485</oboInOwl:id>
        <rdfs:label>Gomez Island</rdfs:label>
    </owl:NamedIndividual>
    


    <!-- http://purl.obolibrary.org/obo/GAZ_00142486 -->

    <owl:NamedIndividual rdf:about="http://purl.obolibrary.org/obo/GAZ_00142486">
        <obo:RO_0001025 rdf:resource="http://purl.obolibrary.org/obo/GAZ_00007175"/>
        <obo:IAO_0000115>Two small islands to the W of Campbell Island.</obo:IAO_0000115>
        <oboInOwl:hasOBONamespace>GAZ</oboInOwl:hasOBONamespace>
        <oboInOwl:id>GAZ:00142486</oboInOwl:id>
        <rdfs:label>Hook Keys</rdfs:label>
    </owl:NamedIndividual>
    


    <!-- http://purl.obolibrary.org/obo/GAZ_00142487 -->

    <owl:NamedIndividual rdf:about="http://purl.obolibrary.org/obo/GAZ_00142487">
        <obo:RO_0001025 rdf:resource="http://purl.obolibrary.org/obo/GAZ_00007175"/>
        <obo:IAO_0000115>A rock to the SW of Monowai Island.</obo:IAO_0000115>
        <oboInOwl:hasOBONamespace>GAZ</oboInOwl:hasOBONamespace>
        <oboInOwl:id>GAZ:00142487</oboInOwl:id>
        <rdfs:label>Seagull Rock</rdfs:label>
    </owl:NamedIndividual>
    


    <!-- http://purl.obolibrary.org/obo/GAZ_00142488 -->

    <owl:NamedIndividual rdf:about="http://purl.obolibrary.org/obo/GAZ_00142488">
        <obo:RO_0001025 rdf:resource="http://purl.obolibrary.org/obo/GAZ_00007175"/>
        <obo:IAO_0000115>An island S of the W peninsula of Campbell Island.</obo:IAO_0000115>
        <oboInOwl:hasOBONamespace>GAZ</oboInOwl:hasOBONamespace>
        <oboInOwl:id>GAZ:00142488</oboInOwl:id>
        <rdfs:label>Survey Island</rdfs:label>
    </owl:NamedIndividual>
    


    <!-- http://purl.obolibrary.org/obo/GAZ_00142489 -->

    <owl:NamedIndividual rdf:about="http://purl.obolibrary.org/obo/GAZ_00142489">
        <obo:RO_0001025 rdf:resource="http://purl.obolibrary.org/obo/GAZ_00007175"/>
        <obo:IAO_0000115>An island to the SW of Campbell Island.</obo:IAO_0000115>
        <oboInOwl:hasOBONamespace>GAZ</oboInOwl:hasOBONamespace>
        <oboInOwl:id>GAZ:00142489</oboInOwl:id>
        <rdfs:label>Wasp Island</rdfs:label>
    </owl:NamedIndividual>
    


    <!-- http://purl.obolibrary.org/obo/GAZ_00142490 -->

    <owl:NamedIndividual rdf:about="http://purl.obolibrary.org/obo/GAZ_00142490">
        <obo:RO_0001025 rdf:resource="http://purl.obolibrary.org/obo/GAZ_00007175"/>
        <obo:IAO_0000115>Rocks NE of Jacquemart Island.</obo:IAO_0000115>
        <oboInOwl:hasOBONamespace>GAZ</oboInOwl:hasOBONamespace>
        <oboInOwl:id>GAZ:00142490</oboInOwl:id>
        <rdfs:label>La Botte</rdfs:label>
    </owl:NamedIndividual>
    


    <!-- http://purl.obolibrary.org/obo/GAZ_00142491 -->

    <owl:NamedIndividual rdf:about="http://purl.obolibrary.org/obo/GAZ_00142491">
        <obo:RO_0001025 rdf:resource="http://purl.obolibrary.org/obo/GAZ_00007175"/>
        <obo:IAO_0000115>A rock off the E of Campbell Island, off the N cape at the entrance to Northeast Harbor.</obo:IAO_0000115>
        <oboInOwl:hasOBONamespace>GAZ</oboInOwl:hasOBONamespace>
        <oboInOwl:id>GAZ:00142491</oboInOwl:id>
        <rdfs:label>Cossack Rock</rdfs:label>
    </owl:NamedIndividual>
    


    <!-- http://purl.obolibrary.org/obo/GAZ_00142492 -->

    <owl:NamedIndividual rdf:about="http://purl.obolibrary.org/obo/GAZ_00142492">
        <rdf:type rdf:resource="http://purl.obolibrary.org/obo/ENVO_00000305"/>
        <obo:RO_0001025 rdf:resource="http://purl.obolibrary.org/obo/GAZ_00017440"/>
        <obo:IAO_0000115>A headland at the end of a long thin peninsula facing S from the southestern peninsula of Campbell Island.</obo:IAO_0000115>
        <oboInOwl:hasOBONamespace>GAZ</oboInOwl:hasOBONamespace>
        <oboInOwl:id>GAZ:00142492</oboInOwl:id>
        <rdfs:label>Shag Point</rdfs:label>
    </owl:NamedIndividual>
    


    <!-- http://purl.obolibrary.org/obo/GAZ_00142493 -->

    <owl:NamedIndividual rdf:about="http://purl.obolibrary.org/obo/GAZ_00142493">
        <rdf:type rdf:resource="http://purl.obolibrary.org/obo/ENVO_00000167"/>
        <obo:RO_0001025 rdf:resource="http://purl.obolibrary.org/obo/GAZ_00017440"/>
        <obo:IAO_0000115>A NW point of Campbell Island.</obo:IAO_0000115>
        <oboInOwl:hasOBONamespace>GAZ</oboInOwl:hasOBONamespace>
        <oboInOwl:id>GAZ:00142493</oboInOwl:id>
        <rdfs:label>Penguin Point</rdfs:label>
    </owl:NamedIndividual>
    


    <!-- http://purl.obolibrary.org/obo/GAZ_00142494 -->

    <owl:NamedIndividual rdf:about="http://purl.obolibrary.org/obo/GAZ_00142494">
        <rdf:type rdf:resource="http://purl.obolibrary.org/obo/ENVO_00000305"/>
        <obo:RO_0001025 rdf:resource="http://purl.obolibrary.org/obo/GAZ_00017440"/>
        <obo:IAO_0000115>A headland on the N of the western peninsula of Campbell Island, marking the W end of Cattle Bay.</obo:IAO_0000115>
        <oboInOwl:hasOBONamespace>GAZ</oboInOwl:hasOBONamespace>
        <oboInOwl:id>GAZ:00142494</oboInOwl:id>
        <rdfs:label>Ramp Point</rdfs:label>
    </owl:NamedIndividual>
    


    <!-- http://purl.obolibrary.org/obo/GAZ_00142495 -->

    <owl:NamedIndividual rdf:about="http://purl.obolibrary.org/obo/GAZ_00142495">
        <rdf:type rdf:resource="http://purl.obolibrary.org/obo/ENVO_00000305"/>
        <obo:RO_0001025 rdf:resource="http://purl.obolibrary.org/obo/GAZ_00017440"/>
        <obo:IAO_0000115>A headland marking the S entrance to Northeast Harbour.</obo:IAO_0000115>
        <oboInOwl:hasOBONamespace>GAZ</oboInOwl:hasOBONamespace>
        <oboInOwl:id>GAZ:00142495</oboInOwl:id>
        <rdfs:label>Cook Point</rdfs:label>
    </owl:NamedIndividual>
    


    <!-- http://purl.obolibrary.org/obo/GAZ_00142496 -->

    <owl:NamedIndividual rdf:about="http://purl.obolibrary.org/obo/GAZ_00142496">
        <rdf:type rdf:resource="http://purl.obolibrary.org/obo/ENVO_00000305"/>
        <obo:RO_0001025 rdf:resource="http://purl.obolibrary.org/obo/GAZ_00017440"/>
        <obo:IAO_0000115>A cape in the NE of Campbell Island.</obo:IAO_0000115>
        <oboInOwl:hasOBONamespace>GAZ</oboInOwl:hasOBONamespace>
        <oboInOwl:id>GAZ:00142496</oboInOwl:id>
        <rdfs:label>North Cape</rdfs:label>
    </owl:NamedIndividual>
    


    <!-- http://purl.obolibrary.org/obo/GAZ_00142497 -->

    <owl:NamedIndividual rdf:about="http://purl.obolibrary.org/obo/GAZ_00142497">
        <rdf:type rdf:resource="http://purl.obolibrary.org/obo/ENVO_00000305"/>
        <obo:RO_0001025 rdf:resource="http://purl.obolibrary.org/obo/GAZ_00017440"/>
        <obo:IAO_0000115>A headland on the N coast of the western peninsula, the W extreme of Northwest Bay.</obo:IAO_0000115>
        <oboInOwl:hasOBONamespace>GAZ</oboInOwl:hasOBONamespace>
        <oboInOwl:id>GAZ:00142497</oboInOwl:id>
        <rdfs:label>Complex Point</rdfs:label>
    </owl:NamedIndividual>
    


    <!-- http://purl.obolibrary.org/obo/GAZ_00142498 -->

    <owl:NamedIndividual rdf:about="http://purl.obolibrary.org/obo/GAZ_00142498">
        <rdf:type rdf:resource="http://purl.obolibrary.org/obo/ENVO_00000305"/>
        <obo:RO_0001025 rdf:resource="http://purl.obolibrary.org/obo/GAZ_00017440"/>
        <obo:IAO_0000115>A headland on the SE peninsula of Campbell Island.</obo:IAO_0000115>
        <oboInOwl:hasOBONamespace>GAZ</oboInOwl:hasOBONamespace>
        <oboInOwl:id>GAZ:00142498</oboInOwl:id>
        <rdfs:label>South Point</rdfs:label>
    </owl:NamedIndividual>
    


    <!-- http://purl.obolibrary.org/obo/GAZ_00142499 -->

    <owl:NamedIndividual rdf:about="http://purl.obolibrary.org/obo/GAZ_00142499">
        <obo:RO_0001025 rdf:resource="http://purl.obolibrary.org/obo/GAZ_00017440"/>
        <obo:IAO_0000115>The E cape of Campbell Island.</obo:IAO_0000115>
        <oboInOwl:hasOBONamespace>GAZ</oboInOwl:hasOBONamespace>
        <oboInOwl:id>GAZ:00142499</oboInOwl:id>
        <rdfs:label>East Cape</rdfs:label>
    </owl:NamedIndividual>
    


    <!-- http://purl.obolibrary.org/obo/GAZ_00142500 -->

    <owl:NamedIndividual rdf:about="http://purl.obolibrary.org/obo/GAZ_00142500">
        <obo:RO_0001025 rdf:resource="http://purl.obolibrary.org/obo/GAZ_00017440"/>
        <obo:IAO_0000115>A S facing point on the E of Campbell Island, facing into Perseverance Harbour.</obo:IAO_0000115>
        <oboInOwl:hasOBONamespace>GAZ</oboInOwl:hasOBONamespace>
        <oboInOwl:id>GAZ:00142500</oboInOwl:id>
        <rdfs:label>Davis Point</rdfs:label>
    </owl:NamedIndividual>
    


    <!-- http://purl.obolibrary.org/obo/GAZ_00142501 -->

    <owl:NamedIndividual rdf:about="http://purl.obolibrary.org/obo/GAZ_00142501">
        <rdf:type rdf:resource="http://purl.obolibrary.org/obo/ENVO_00000305"/>
        <obo:RO_0001025 rdf:resource="http://purl.obolibrary.org/obo/GAZ_00017440"/>
        <obo:IAO_0000115>A headland on the E of Campbell Island, S of Cook Point.</obo:IAO_0000115>
        <oboInOwl:hasOBONamespace>GAZ</oboInOwl:hasOBONamespace>
        <oboInOwl:id>GAZ:00142501</oboInOwl:id>
        <rdfs:label>Macdonald Point</rdfs:label>
    </owl:NamedIndividual>
    


    <!-- http://purl.obolibrary.org/obo/GAZ_00142502 -->

    <owl:NamedIndividual rdf:about="http://purl.obolibrary.org/obo/GAZ_00142502">
        <obo:RO_0001025 rdf:resource="http://purl.obolibrary.org/obo/GAZ_00017440"/>
        <obo:IAO_0000115>A lake on the S of Campbell Island connecting to and N of Monument Harbour.</obo:IAO_0000115>
        <oboInOwl:hasOBONamespace>GAZ</oboInOwl:hasOBONamespace>
        <oboInOwl:id>GAZ:00142502</oboInOwl:id>
        <rdfs:label>Six Foot Lake</rdfs:label>
    </owl:NamedIndividual>
    


    <!-- http://purl.obolibrary.org/obo/GAZ_00142508 -->

    <owl:NamedIndividual rdf:about="http://purl.obolibrary.org/obo/GAZ_00142508">
        <obo:RO_0001025 rdf:resource="http://purl.obolibrary.org/obo/GAZ_00017440"/>
        <obo:IAO_0000115>A headland projecting into the head of Perseverance Harbour.</obo:IAO_0000115>
        <oboInOwl:hasOBONamespace>GAZ</oboInOwl:hasOBONamespace>
        <oboInOwl:id>GAZ:00142508</oboInOwl:id>
        <rdfs:label>Duris Point</rdfs:label>
    </owl:NamedIndividual>
    


    <!-- http://purl.obolibrary.org/obo/GAZ_00142509 -->

    <owl:NamedIndividual rdf:about="http://purl.obolibrary.org/obo/GAZ_00142509">
        <obo:RO_0001025 rdf:resource="http://purl.obolibrary.org/obo/GAZ_00017440"/>
        <obo:IAO_0000115>A stream running into Northeast Harbour.</obo:IAO_0000115>
        <oboInOwl:hasOBONamespace>GAZ</oboInOwl:hasOBONamespace>
        <oboInOwl:id>GAZ:00142509</oboInOwl:id>
        <rdfs:label>Northeast Stream</rdfs:label>
    </owl:NamedIndividual>
    


    <!-- http://purl.obolibrary.org/obo/GAZ_00142510 -->

    <owl:NamedIndividual rdf:about="http://purl.obolibrary.org/obo/GAZ_00142510">
        <obo:RO_0001025 rdf:resource="http://purl.obolibrary.org/obo/GAZ_00017440"/>
        <obo:IAO_0000115>A stream running into the head of Perserverance Harbour.</obo:IAO_0000115>
        <oboInOwl:hasOBONamespace>GAZ</oboInOwl:hasOBONamespace>
        <oboInOwl:id>GAZ:00142510</oboInOwl:id>
        <rdfs:label>Camp Stream</rdfs:label>
    </owl:NamedIndividual>
    


    <!-- http://purl.obolibrary.org/obo/GAZ_00142511 -->

    <owl:NamedIndividual rdf:about="http://purl.obolibrary.org/obo/GAZ_00142511">
        <rdf:type rdf:resource="http://purl.obolibrary.org/obo/ENVO_00000305"/>
        <obo:RO_0001025 rdf:resource="http://purl.obolibrary.org/obo/GAZ_00017440"/>
        <obo:IAO_0000115>A headland on the N shore of Perserverance Harbour.</obo:IAO_0000115>
        <oboInOwl:hasOBONamespace>GAZ</oboInOwl:hasOBONamespace>
        <oboInOwl:id>GAZ:00142511</oboInOwl:id>
        <rdfs:label>Beeman Point</rdfs:label>
    </owl:NamedIndividual>
    


    <!-- http://purl.obolibrary.org/obo/GAZ_00142512 -->

    <owl:NamedIndividual rdf:about="http://purl.obolibrary.org/obo/GAZ_00142512">
        <rdf:type rdf:resource="http://purl.obolibrary.org/obo/ENVO_00000167"/>
        <obo:RO_0001025 rdf:resource="http://purl.obolibrary.org/obo/GAZ_00017440"/>
        <obo:IAO_0000115>A small point on the N shore of Perserverance Harbour.</obo:IAO_0000115>
        <oboInOwl:hasOBONamespace>GAZ</oboInOwl:hasOBONamespace>
        <oboInOwl:id>GAZ:00142512</oboInOwl:id>
        <rdfs:label>Boyack Point</rdfs:label>
    </owl:NamedIndividual>
    


    <!-- http://purl.obolibrary.org/obo/GAZ_00142513 -->

    <owl:NamedIndividual rdf:about="http://purl.obolibrary.org/obo/GAZ_00142513">
        <rdf:type rdf:resource="http://purl.obolibrary.org/obo/ENVO_00000305"/>
        <obo:RO_0001025 rdf:resource="http://purl.obolibrary.org/obo/GAZ_00017440"/>
        <obo:IAO_0000115>A headland at the end of a blunt peninsula into the head of Perserverance Harbor, on the N shore.</obo:IAO_0000115>
        <oboInOwl:hasOBONamespace>GAZ</oboInOwl:hasOBONamespace>
        <oboInOwl:id>GAZ:00142513</oboInOwl:id>
        <rdfs:label>Depot Point</rdfs:label>
    </owl:NamedIndividual>
    


    <!-- http://purl.obolibrary.org/obo/GAZ_00142514 -->

    <owl:NamedIndividual rdf:about="http://purl.obolibrary.org/obo/GAZ_00142514">
        <obo:RO_0001025 rdf:resource="http://purl.obolibrary.org/obo/GAZ_00017440"/>
        <obo:IAO_0000115>A stream S of Mount Faye and Faye Bump running into the sea on the E shore of the northeast peninsula of Campbell Island.</obo:IAO_0000115>
        <oboInOwl:hasOBONamespace>GAZ</oboInOwl:hasOBONamespace>
        <oboInOwl:id>GAZ:00142514</oboInOwl:id>
        <rdfs:label>Buchanan Stream</rdfs:label>
    </owl:NamedIndividual>
    


    <!-- http://purl.obolibrary.org/obo/GAZ_00142515 -->

    <owl:NamedIndividual rdf:about="http://purl.obolibrary.org/obo/GAZ_00142515">
        <obo:RO_0001025 rdf:resource="http://purl.obolibrary.org/obo/GAZ_00017440"/>
        <obo:IAO_0000115>A stream runng into the sea at the N end of the northeastern peninsula of Campbell Island.</obo:IAO_0000115>
        <oboInOwl:hasOBONamespace>GAZ</oboInOwl:hasOBONamespace>
        <oboInOwl:id>GAZ:00142515</oboInOwl:id>
        <rdfs:label>Twin Falls Stream</rdfs:label>
    </owl:NamedIndividual>
    


    <!-- http://purl.obolibrary.org/obo/GAZ_00142516 -->

    <owl:NamedIndividual rdf:about="http://purl.obolibrary.org/obo/GAZ_00142516">
        <obo:RO_0001025 rdf:resource="http://purl.obolibrary.org/obo/GAZ_00017440"/>
        <obo:IAO_0000115>A stream entering the N end of Smoothwater Bay.</obo:IAO_0000115>
        <oboInOwl:hasOBONamespace>GAZ</oboInOwl:hasOBONamespace>
        <oboInOwl:id>GAZ:00142516</oboInOwl:id>
        <rdfs:label>Smoothwater Stream</rdfs:label>
    </owl:NamedIndividual>
    


    <!-- http://purl.obolibrary.org/obo/GAZ_00142517 -->

    <owl:NamedIndividual rdf:about="http://purl.obolibrary.org/obo/GAZ_00142517">
        <obo:RO_0001025 rdf:resource="http://purl.obolibrary.org/obo/GAZ_00017440"/>
        <obo:IAO_0000115>A stream on the southeastern peninsula of Campbell Island, entering the sea just W of the peninsula that ends in Shag Point.</obo:IAO_0000115>
        <oboInOwl:hasOBONamespace>GAZ</oboInOwl:hasOBONamespace>
        <oboInOwl:id>GAZ:00142517</oboInOwl:id>
        <rdfs:label>Shag Stream</rdfs:label>
    </owl:NamedIndividual>
    


    <!-- http://purl.obolibrary.org/obo/GAZ_00142518 -->

    <owl:NamedIndividual rdf:about="http://purl.obolibrary.org/obo/GAZ_00142518">
        <obo:RO_0001025 rdf:resource="http://purl.obolibrary.org/obo/GAZ_00017440"/>
        <obo:IAO_0000115>A stream on the S of Campbell Island, entering Southeast Harbour.</obo:IAO_0000115>
        <oboInOwl:hasOBONamespace>GAZ</oboInOwl:hasOBONamespace>
        <oboInOwl:id>GAZ:00142518</oboInOwl:id>
        <rdfs:label>Southeast Stream</rdfs:label>
    </owl:NamedIndividual>
    


    <!-- http://purl.obolibrary.org/obo/GAZ_00142519 -->

    <owl:NamedIndividual rdf:about="http://purl.obolibrary.org/obo/GAZ_00142519">
        <obo:RO_0001025 rdf:resource="http://purl.obolibrary.org/obo/GAZ_00017440"/>
        <obo:IAO_0000115>A stream entering Six Foot Lake in its NW.</obo:IAO_0000115>
        <oboInOwl:hasOBONamespace>GAZ</oboInOwl:hasOBONamespace>
        <oboInOwl:id>GAZ:00142519</oboInOwl:id>
        <rdfs:label>Kirk Stream</rdfs:label>
    </owl:NamedIndividual>
    


    <!-- http://purl.obolibrary.org/obo/GAZ_00142520 -->

    <owl:NamedIndividual rdf:about="http://purl.obolibrary.org/obo/GAZ_00142520">
        <obo:RO_0001025 rdf:resource="http://purl.obolibrary.org/obo/GAZ_00017440"/>
        <obo:IAO_0000115>A N running stream entering the head of Perseverance Bay.</obo:IAO_0000115>
        <oboInOwl:hasOBONamespace>GAZ</oboInOwl:hasOBONamespace>
        <oboInOwl:id>GAZ:00142520</oboInOwl:id>
        <rdfs:label>Garden Stream</rdfs:label>
    </owl:NamedIndividual>
    


    <!-- http://purl.obolibrary.org/obo/GAZ_00142521 -->

    <owl:NamedIndividual rdf:about="http://purl.obolibrary.org/obo/GAZ_00142521">
        <obo:RO_0001025 rdf:resource="http://purl.obolibrary.org/obo/GAZ_00017440"/>
        <obo:IAO_0000115>A NE running stream entering the head of Perseverance Bay.</obo:IAO_0000115>
        <oboInOwl:hasOBONamespace>GAZ</oboInOwl:hasOBONamespace>
        <oboInOwl:id>GAZ:00142521</oboInOwl:id>
        <rdfs:label>Dumes Stream</rdfs:label>
    </owl:NamedIndividual>
    


    <!-- http://purl.obolibrary.org/obo/GAZ_00142522 -->

    <owl:NamedIndividual rdf:about="http://purl.obolibrary.org/obo/GAZ_00142522">
        <obo:RO_0001025 rdf:resource="http://purl.obolibrary.org/obo/GAZ_00017440"/>
        <obo:IAO_0000115>A stream entering the W end of Northwest Bay.</obo:IAO_0000115>
        <oboInOwl:hasOBONamespace>GAZ</oboInOwl:hasOBONamespace>
        <oboInOwl:id>GAZ:00142522</oboInOwl:id>
        <rdfs:label>Norton Stream</rdfs:label>
    </owl:NamedIndividual>
    


    <!-- http://purl.obolibrary.org/obo/GAZ_00142523 -->

    <owl:NamedIndividual rdf:about="http://purl.obolibrary.org/obo/GAZ_00142523">
        <obo:RO_0001025 rdf:resource="http://purl.obolibrary.org/obo/GAZ_00007126"/>
        <obo:IAO_0000115>A very small island off the NE coast of Pitt Island.</obo:IAO_0000115>
        <oboInOwl:hasOBONamespace>GAZ</oboInOwl:hasOBONamespace>
        <oboInOwl:id>GAZ:00142523</oboInOwl:id>
        <rdfs:label>Kokopa</rdfs:label>
    </owl:NamedIndividual>
    


    <!-- http://purl.obolibrary.org/obo/GAZ_00142524 -->

    <owl:NamedIndividual rdf:about="http://purl.obolibrary.org/obo/GAZ_00142524">
        <obo:RO_0001025 rdf:resource="http://purl.obolibrary.org/obo/GAZ_00007126"/>
        <obo:IAO_0000115>A rock to the SW of Pitt Island.</obo:IAO_0000115>
        <oboInOwl:hasOBONamespace>GAZ</oboInOwl:hasOBONamespace>
        <oboInOwl:id>GAZ:00142524</oboInOwl:id>
        <rdfs:label>Round Rock</rdfs:label>
    </owl:NamedIndividual>
    


    <!-- http://purl.obolibrary.org/obo/GAZ_00142525 -->

    <owl:NamedIndividual rdf:about="http://purl.obolibrary.org/obo/GAZ_00142525">
        <obo:RO_0001025 rdf:resource="http://purl.obolibrary.org/obo/GAZ_00007126"/>
        <obo:IAO_0000115>Rocks off the SW of Chatham Island, S of Cape Fournier.</obo:IAO_0000115>
        <oboInOwl:hasOBONamespace>GAZ</oboInOwl:hasOBONamespace>
        <oboInOwl:id>GAZ:00142525</oboInOwl:id>
        <rdfs:label>Tapuaranga Reef</rdfs:label>
    </owl:NamedIndividual>
    


    <!-- http://purl.obolibrary.org/obo/GAZ_00142526 -->

    <owl:NamedIndividual rdf:about="http://purl.obolibrary.org/obo/GAZ_00142526">
        <obo:RO_0001025 rdf:resource="http://purl.obolibrary.org/obo/GAZ_00007126"/>
        <obo:IAO_0000115>A small rock SE of South East Island.</obo:IAO_0000115>
        <oboInOwl:hasOBONamespace>GAZ</oboInOwl:hasOBONamespace>
        <oboInOwl:id>GAZ:00142526</oboInOwl:id>
        <rdfs:label>Fancy Rock</rdfs:label>
    </owl:NamedIndividual>
    


    <!-- http://purl.obolibrary.org/obo/GAZ_00142527 -->

    <owl:NamedIndividual rdf:about="http://purl.obolibrary.org/obo/GAZ_00142527">
        <obo:RO_0001025 rdf:resource="http://purl.obolibrary.org/obo/GAZ_00007126"/>
        <obo:IAO_0000115>A small island SE of Mangere Island.</obo:IAO_0000115>
        <oboInOwl:hasOBONamespace>GAZ</oboInOwl:hasOBONamespace>
        <oboInOwl:id>GAZ:00142527</oboInOwl:id>
        <rdfs:label>Sugar Loaf</rdfs:label>
    </owl:NamedIndividual>
    


    <!-- http://purl.obolibrary.org/obo/GAZ_00142529 -->

    <owl:NamedIndividual rdf:about="http://purl.obolibrary.org/obo/GAZ_00142529">
        <obo:RO_0001025 rdf:resource="http://purl.obolibrary.org/obo/GAZ_00007126"/>
        <obo:IAO_0000115>An island of Tarawhenua Point, Pitt Island.</obo:IAO_0000115>
        <oboInOwl:hasOBONamespace>GAZ</oboInOwl:hasOBONamespace>
        <oboInOwl:id>GAZ:00142529</oboInOwl:id>
        <rdfs:label>Rabbit Island</rdfs:label>
    </owl:NamedIndividual>
    


    <!-- http://purl.obolibrary.org/obo/GAZ_00142530 -->

    <owl:NamedIndividual rdf:about="http://purl.obolibrary.org/obo/GAZ_00142530">
        <obo:RO_0001025 rdf:resource="http://purl.obolibrary.org/obo/GAZ_00007126"/>
        <obo:IAO_0000115>Reefs E of Kahuitara Point of Pitt Island.</obo:IAO_0000115>
        <oboInOwl:hasOBONamespace>GAZ</oboInOwl:hasOBONamespace>
        <oboInOwl:id>GAZ:00142530</oboInOwl:id>
        <rdfs:label>North East Reef</rdfs:label>
    </owl:NamedIndividual>
    


    <!-- http://purl.obolibrary.org/obo/GAZ_00142531 -->

    <owl:NamedIndividual rdf:about="http://purl.obolibrary.org/obo/GAZ_00142531">
        <obo:RO_0001025 rdf:resource="http://purl.obolibrary.org/obo/GAZ_00007126"/>
        <obo:IAO_0000115>A rock between Pitt Island and South East Island.</obo:IAO_0000115>
        <oboInOwl:hasOBONamespace>GAZ</oboInOwl:hasOBONamespace>
        <oboInOwl:id>GAZ:00142531</oboInOwl:id>
        <rdfs:label>Passage Rock</rdfs:label>
    </owl:NamedIndividual>
    


    <!-- http://purl.obolibrary.org/obo/GAZ_00142532 -->

    <owl:NamedIndividual rdf:about="http://purl.obolibrary.org/obo/GAZ_00142532">
        <obo:RO_0001025 rdf:resource="http://purl.obolibrary.org/obo/GAZ_00016318"/>
        <obo:IAO_0000115>A S point of Chatham Island.</obo:IAO_0000115>
        <oboInOwl:hasOBONamespace>GAZ</oboInOwl:hasOBONamespace>
        <oboInOwl:id>GAZ:00142532</oboInOwl:id>
        <rdfs:label>Green Point</rdfs:label>
    </owl:NamedIndividual>
    


    <!-- http://purl.obolibrary.org/obo/GAZ_00142533 -->

    <owl:NamedIndividual rdf:about="http://purl.obolibrary.org/obo/GAZ_00142533">
        <rdf:type rdf:resource="http://purl.obolibrary.org/obo/ENVO_00000305"/>
        <obo:RO_0001025 rdf:resource="http://purl.obolibrary.org/obo/GAZ_00016316"/>
        <obo:IAO_0000115>A headland at the end of a small peninsula in the SW of Pitt Island.</obo:IAO_0000115>
        <oboInOwl:hasOBONamespace>GAZ</oboInOwl:hasOBONamespace>
        <oboInOwl:id>GAZ:00142533</oboInOwl:id>
        <rdfs:label>Rangiauria Point</rdfs:label>
    </owl:NamedIndividual>
    


    <!-- http://purl.obolibrary.org/obo/GAZ_00142534 -->

    <owl:NamedIndividual rdf:about="http://purl.obolibrary.org/obo/GAZ_00142534">
        <obo:RO_0001025 rdf:resource="http://purl.obolibrary.org/obo/GAZ_00016316"/>
        <obo:IAO_0000115>The E point of Pitt Island, at the end of a short peninsula.</obo:IAO_0000115>
        <oboInOwl:hasOBONamespace>GAZ</oboInOwl:hasOBONamespace>
        <oboInOwl:id>GAZ:00142534</oboInOwl:id>
        <rdfs:label>Kahuitara Point</rdfs:label>
    </owl:NamedIndividual>
    


    <!-- http://purl.obolibrary.org/obo/GAZ_00142535 -->

    <owl:NamedIndividual rdf:about="http://purl.obolibrary.org/obo/GAZ_00142535">
        <obo:RO_0001025 rdf:resource="http://purl.obolibrary.org/obo/GAZ_00016316"/>
        <obo:IAO_0000115>The N point of Pitt Island.</obo:IAO_0000115>
        <oboInOwl:hasOBONamespace>GAZ</oboInOwl:hasOBONamespace>
        <oboInOwl:id>GAZ:00142535</oboInOwl:id>
        <rdfs:label>Motutapu Point</rdfs:label>
    </owl:NamedIndividual>
    


    <!-- http://purl.obolibrary.org/obo/GAZ_00142536 -->

    <owl:NamedIndividual rdf:about="http://purl.obolibrary.org/obo/GAZ_00142536">
        <obo:RO_0001025 rdf:resource="http://purl.obolibrary.org/obo/GAZ_00016316"/>
        <obo:IAO_0000115>A E flowing stream on Pitt Island.</obo:IAO_0000115>
        <oboInOwl:hasOBONamespace>GAZ</oboInOwl:hasOBONamespace>
        <oboInOwl:id>GAZ:00142536</oboInOwl:id>
        <rdfs:label>Second Water Creek</rdfs:label>
    </owl:NamedIndividual>
    


    <!-- http://purl.obolibrary.org/obo/GAZ_00142537 -->

    <owl:NamedIndividual rdf:about="http://purl.obolibrary.org/obo/GAZ_00142537">
        <obo:RO_0001025 rdf:resource="http://purl.obolibrary.org/obo/GAZ_00016316"/>
        <obo:IAO_0000115>An E flowing stream on Pitt Island.</obo:IAO_0000115>
        <oboInOwl:hasOBONamespace>GAZ</oboInOwl:hasOBONamespace>
        <oboInOwl:id>GAZ:00142537</oboInOwl:id>
        <rdfs:label>Waipaua Stream</rdfs:label>
    </owl:NamedIndividual>
    


    <!-- http://purl.obolibrary.org/obo/GAZ_00142538 -->

    <owl:NamedIndividual rdf:about="http://purl.obolibrary.org/obo/GAZ_00142538">
        <obo:RO_0001025 rdf:resource="http://purl.obolibrary.org/obo/GAZ_00016316"/>
        <obo:IAO_0000115>The NW point of Pitt Island.</obo:IAO_0000115>
        <oboInOwl:hasOBONamespace>GAZ</oboInOwl:hasOBONamespace>
        <oboInOwl:id>GAZ:00142538</oboInOwl:id>
        <rdfs:label>Tarawhenua Point</rdfs:label>
    </owl:NamedIndividual>
    


    <!-- http://purl.obolibrary.org/obo/GAZ_00142547 -->

    <owl:NamedIndividual rdf:about="http://purl.obolibrary.org/obo/GAZ_00142547">
        <rdf:type rdf:resource="http://purl.obolibrary.org/obo/ENVO_00000305"/>
        <obo:RO_0001025 rdf:resource="http://purl.obolibrary.org/obo/GAZ_00016318"/>
        <obo:IAO_0000115>A headland in the northwest of Chatham Island, the largest island in the Chatham Islands chain, located 800 km east of New Zealand&apos;s South Island.</obo:IAO_0000115>
        <oboInOwl:hasOBONamespace>GAZ</oboInOwl:hasOBONamespace>
        <oboInOwl:id>GAZ:00142547</oboInOwl:id>
        <rdfs:label>Cape Pattison</rdfs:label>
    </owl:NamedIndividual>
    


    <!-- http://purl.obolibrary.org/obo/GAZ_00142548 -->

    <owl:NamedIndividual rdf:about="http://purl.obolibrary.org/obo/GAZ_00142548">
        <obo:RO_0001025 rdf:resource="http://purl.obolibrary.org/obo/GAZ_00007126"/>
        <obo:IAO_0000115>A reef N of Point Durham.</obo:IAO_0000115>
        <oboInOwl:hasOBONamespace>GAZ</oboInOwl:hasOBONamespace>
        <oboInOwl:id>GAZ:00142548</oboInOwl:id>
        <rdfs:label>Jenny Reef</rdfs:label>
    </owl:NamedIndividual>
    


    <!-- http://purl.obolibrary.org/obo/GAZ_00142549 -->

    <owl:NamedIndividual rdf:about="http://purl.obolibrary.org/obo/GAZ_00142549">
        <obo:RO_0001025 rdf:resource="http://purl.obolibrary.org/obo/GAZ_00007126"/>
        <obo:IAO_0000115>A small rock off the SE coast of Chatham Island.</obo:IAO_0000115>
        <oboInOwl:hasOBONamespace>GAZ</oboInOwl:hasOBONamespace>
        <oboInOwl:id>GAZ:00142549</oboInOwl:id>
        <rdfs:label>Boundary Rock</rdfs:label>
    </owl:NamedIndividual>
    


    <!-- http://purl.obolibrary.org/obo/GAZ_00142550 -->

    <owl:NamedIndividual rdf:about="http://purl.obolibrary.org/obo/GAZ_00142550">
        <obo:RO_0001025 rdf:resource="http://purl.obolibrary.org/obo/GAZ_00007126"/>
        <obo:IAO_0000115>In shore rocks off the SE coast of Chatham Island.</obo:IAO_0000115>
        <oboInOwl:hasOBONamespace>GAZ</oboInOwl:hasOBONamespace>
        <oboInOwl:id>GAZ:00142550</oboInOwl:id>
        <rdfs:label>The Pinnacles</rdfs:label>
    </owl:NamedIndividual>
    


    <!-- http://purl.obolibrary.org/obo/GAZ_00142551 -->

    <owl:NamedIndividual rdf:about="http://purl.obolibrary.org/obo/GAZ_00142551">
        <obo:RO_0001025 rdf:resource="http://purl.obolibrary.org/obo/GAZ_00007126"/>
        <obo:IAO_0000115>An in shore island off SE Chatham Island, N of Cascade Gorge.</obo:IAO_0000115>
        <oboInOwl:hasOBONamespace>GAZ</oboInOwl:hasOBONamespace>
        <oboInOwl:id>GAZ:00142551</oboInOwl:id>
        <rdfs:label>Houruekopara Island</rdfs:label>
    </owl:NamedIndividual>
    


    <!-- http://purl.obolibrary.org/obo/GAZ_00142552 -->

    <owl:NamedIndividual rdf:about="http://purl.obolibrary.org/obo/GAZ_00142552">
        <obo:RO_0001025 rdf:resource="http://purl.obolibrary.org/obo/GAZ_00007126"/>
        <obo:IAO_0000115>A rock off the SE of Chatham Island, NE of Ko Oreao Point.</obo:IAO_0000115>
        <oboInOwl:hasOBONamespace>GAZ</oboInOwl:hasOBONamespace>
        <oboInOwl:id>GAZ:00142552</oboInOwl:id>
        <rdfs:label>Te Awatapu Rock</rdfs:label>
    </owl:NamedIndividual>
    


    <!-- http://purl.obolibrary.org/obo/GAZ_00142553 -->

    <owl:NamedIndividual rdf:about="http://purl.obolibrary.org/obo/GAZ_00142553">
        <rdf:type rdf:resource="http://purl.obolibrary.org/obo/ENVO_00000167"/>
        <obo:RO_0001025 rdf:resource="http://purl.obolibrary.org/obo/GAZ_00007126"/>
        <obo:IAO_0000115>A shoal in Hansen Bay, just SE of the Hikurangi Channel.</obo:IAO_0000115>
        <oboInOwl:hasOBONamespace>GAZ</oboInOwl:hasOBONamespace>
        <oboInOwl:id>GAZ:00142553</oboInOwl:id>
        <rdfs:label>Tokatapu Shoal</rdfs:label>
    </owl:NamedIndividual>
    


    <!-- http://purl.obolibrary.org/obo/GAZ_00142554 -->

    <owl:NamedIndividual rdf:about="http://purl.obolibrary.org/obo/GAZ_00142554">
        <obo:RO_0001025 rdf:resource="http://purl.obolibrary.org/obo/GAZ_00007126"/>
        <obo:IAO_0000115>A reef, SE of Boundary Rock, off the SE of Chatham Island.</obo:IAO_0000115>
        <oboInOwl:hasOBONamespace>GAZ</oboInOwl:hasOBONamespace>
        <oboInOwl:id>GAZ:00142554</oboInOwl:id>
        <rdfs:label>Renweeks Reef</rdfs:label>
    </owl:NamedIndividual>
    


    <!-- http://purl.obolibrary.org/obo/GAZ_00142555 -->

    <owl:NamedIndividual rdf:about="http://purl.obolibrary.org/obo/GAZ_00142555">
        <rdf:type rdf:resource="http://purl.obolibrary.org/obo/ENVO_00000020"/>
        <obo:RO_0001025 rdf:resource="http://purl.obolibrary.org/obo/GAZ_00007126"/>
        <obo:IAO_0000115>A broad in shore shoal off the NW coast of the S part of Chatham Island, SW of Kahunana Point.</obo:IAO_0000115>
        <oboInOwl:hasOBONamespace>GAZ</oboInOwl:hasOBONamespace>
        <oboInOwl:id>GAZ:00142555</oboInOwl:id>
        <rdfs:label>Heephy Shoal</rdfs:label>
    </owl:NamedIndividual>
    


    <!-- http://purl.obolibrary.org/obo/GAZ_00142556 -->

    <owl:NamedIndividual rdf:about="http://purl.obolibrary.org/obo/GAZ_00142556">
        <obo:RO_0001025 rdf:resource="http://purl.obolibrary.org/obo/GAZ_00007126"/>
        <obo:IAO_0000115>An in shore reef off Point Weeding.</obo:IAO_0000115>
        <oboInOwl:hasOBONamespace>GAZ</oboInOwl:hasOBONamespace>
        <oboInOwl:id>GAZ:00142556</oboInOwl:id>
        <rdfs:label>McClatchie Reef</rdfs:label>
    </owl:NamedIndividual>
    


    <!-- http://purl.obolibrary.org/obo/GAZ_00142557 -->

    <owl:NamedIndividual rdf:about="http://purl.obolibrary.org/obo/GAZ_00142557">
        <obo:RO_0001025 rdf:resource="http://purl.obolibrary.org/obo/GAZ_00007126"/>
        <obo:IAO_0000115>A rock in the W of Chatham Island, NE of Point Durham.</obo:IAO_0000115>
        <oboInOwl:hasOBONamespace>GAZ</oboInOwl:hasOBONamespace>
        <oboInOwl:id>GAZ:00142557</oboInOwl:id>
        <rdfs:label>Turange Rock</rdfs:label>
    </owl:NamedIndividual>
    


    <!-- http://purl.obolibrary.org/obo/GAZ_00142558 -->

    <owl:NamedIndividual rdf:about="http://purl.obolibrary.org/obo/GAZ_00142558">
        <obo:RO_0001025 rdf:resource="http://purl.obolibrary.org/obo/GAZ_00016318"/>
        <obo:IAO_0000115>The SW point of Chatham Island.</obo:IAO_0000115>
        <oboInOwl:hasOBONamespace>GAZ</oboInOwl:hasOBONamespace>
        <oboInOwl:id>GAZ:00142558</oboInOwl:id>
        <rdfs:label>Cape Fournier</rdfs:label>
    </owl:NamedIndividual>
    


    <!-- http://purl.obolibrary.org/obo/GAZ_00142565 -->

    <owl:NamedIndividual rdf:about="http://purl.obolibrary.org/obo/GAZ_00142565">
        <obo:RO_0001025 rdf:resource="http://purl.obolibrary.org/obo/GAZ_00016318"/>
        <obo:IAO_0000115>The point at the end of a short triangular-shaped peninsula in SE Chatham Island.</obo:IAO_0000115>
        <oboInOwl:hasOBONamespace>GAZ</oboInOwl:hasOBONamespace>
        <oboInOwl:id>GAZ:00142565</oboInOwl:id>
        <rdfs:label>Ko Oreao Point</rdfs:label>
    </owl:NamedIndividual>
    


    <!-- http://purl.obolibrary.org/obo/GAZ_00142566 -->

    <owl:NamedIndividual rdf:about="http://purl.obolibrary.org/obo/GAZ_00142566">
        <rdf:type rdf:resource="http://purl.obolibrary.org/obo/ENVO_00000100"/>
        <obo:RO_0001025 rdf:resource="http://purl.obolibrary.org/obo/GAZ_00016318"/>
        <obo:IAO_0000115>A gorge in SE Chatham Island.</obo:IAO_0000115>
        <oboInOwl:hasOBONamespace>GAZ</oboInOwl:hasOBONamespace>
        <oboInOwl:id>GAZ:00142566</oboInOwl:id>
        <rdfs:label>Cascade Gorge</rdfs:label>
    </owl:NamedIndividual>
    


    <!-- http://purl.obolibrary.org/obo/GAZ_00142567 -->

    <owl:NamedIndividual rdf:about="http://purl.obolibrary.org/obo/GAZ_00142567">
        <obo:RO_0001025 rdf:resource="http://purl.obolibrary.org/obo/GAZ_00016318"/>
        <obo:IAO_0000115>The SW cape of Chatham Island.</obo:IAO_0000115>
        <oboInOwl:hasOBONamespace>GAZ</oboInOwl:hasOBONamespace>
        <oboInOwl:id>GAZ:00142567</oboInOwl:id>
        <rdfs:label>Cape L&apos;Eveque</rdfs:label>
    </owl:NamedIndividual>
    


    <!-- http://purl.obolibrary.org/obo/GAZ_00142568 -->

    <owl:NamedIndividual rdf:about="http://purl.obolibrary.org/obo/GAZ_00142568">
        <obo:RO_0001025 rdf:resource="http://purl.obolibrary.org/obo/GAZ_00016318"/>
        <obo:IAO_0000115>A lake in the S of Chatham Island.</obo:IAO_0000115>
        <oboInOwl:hasOBONamespace>GAZ</oboInOwl:hasOBONamespace>
        <oboInOwl:id>GAZ:00142568</oboInOwl:id>
        <rdfs:label>Lake Tuku a taupo</rdfs:label>
    </owl:NamedIndividual>
    


    <!-- http://purl.obolibrary.org/obo/GAZ_00142569 -->

    <owl:NamedIndividual rdf:about="http://purl.obolibrary.org/obo/GAZ_00142569">
        <rdf:type rdf:resource="http://purl.obolibrary.org/obo/ENVO_00000305"/>
        <obo:RO_0001025 rdf:resource="http://purl.obolibrary.org/obo/GAZ_00016318"/>
        <obo:IAO_0000115>A headland on the NW side of the peninsula that ends in Cape L&apos;Eveque.</obo:IAO_0000115>
        <oboInOwl:hasOBONamespace>GAZ</oboInOwl:hasOBONamespace>
        <oboInOwl:id>GAZ:00142569</oboInOwl:id>
        <rdfs:label>Te Whakahewa</rdfs:label>
    </owl:NamedIndividual>
    


    <!-- http://purl.obolibrary.org/obo/GAZ_00142570 -->

    <owl:NamedIndividual rdf:about="http://purl.obolibrary.org/obo/GAZ_00142570">
        <rdf:type rdf:resource="http://purl.obolibrary.org/obo/ENVO_00000305"/>
        <obo:RO_0001025 rdf:resource="http://purl.obolibrary.org/obo/GAZ_00016318"/>
        <obo:IAO_0000115>A headland on the SW coast of Chatham Island.</obo:IAO_0000115>
        <oboInOwl:hasOBONamespace>GAZ</oboInOwl:hasOBONamespace>
        <oboInOwl:id>GAZ:00142570</oboInOwl:id>
        <rdfs:label>Point Gap</rdfs:label>
    </owl:NamedIndividual>
    


    <!-- http://purl.obolibrary.org/obo/GAZ_00142571 -->

    <owl:NamedIndividual rdf:about="http://purl.obolibrary.org/obo/GAZ_00142571">
        <obo:RO_0001025 rdf:resource="http://purl.obolibrary.org/obo/GAZ_00016318"/>
        <obo:IAO_0000115>A lake in the S of Chatham Island.</obo:IAO_0000115>
        <oboInOwl:hasOBONamespace>GAZ</oboInOwl:hasOBONamespace>
        <oboInOwl:id>GAZ:00142571</oboInOwl:id>
        <rdfs:label>Lake Pukawa</rdfs:label>
    </owl:NamedIndividual>
    


    <!-- http://purl.obolibrary.org/obo/GAZ_00142572 -->

    <owl:NamedIndividual rdf:about="http://purl.obolibrary.org/obo/GAZ_00142572">
        <obo:RO_0001025 rdf:resource="http://purl.obolibrary.org/obo/GAZ_00016318"/>
        <obo:IAO_0000115>A W point on the S part of Chatham Island.</obo:IAO_0000115>
        <oboInOwl:hasOBONamespace>GAZ</oboInOwl:hasOBONamespace>
        <oboInOwl:id>GAZ:00142572</oboInOwl:id>
        <rdfs:label>Point Durham</rdfs:label>
    </owl:NamedIndividual>
    


    <!-- http://purl.obolibrary.org/obo/GAZ_00142573 -->

    <owl:NamedIndividual rdf:about="http://purl.obolibrary.org/obo/GAZ_00142573">
        <obo:RO_0001025 rdf:resource="http://purl.obolibrary.org/obo/GAZ_00016318"/>
        <obo:IAO_0000115>A lake in the S of Chatham Island.</obo:IAO_0000115>
        <oboInOwl:hasOBONamespace>GAZ</oboInOwl:hasOBONamespace>
        <oboInOwl:id>GAZ:00142573</oboInOwl:id>
        <rdfs:label>Lake Matangirau</rdfs:label>
    </owl:NamedIndividual>
    


    <!-- http://purl.obolibrary.org/obo/GAZ_00142574 -->

    <owl:NamedIndividual rdf:about="http://purl.obolibrary.org/obo/GAZ_00142574">
        <rdf:type rdf:resource="http://purl.obolibrary.org/obo/ENVO_00000167"/>
        <obo:RO_0001025 rdf:resource="http://purl.obolibrary.org/obo/GAZ_00016318"/>
        <obo:IAO_0000115>A SW point of Chatham Island, N of Cape L&apos;Eveque.</obo:IAO_0000115>
        <oboInOwl:hasOBONamespace>GAZ</oboInOwl:hasOBONamespace>
        <oboInOwl:id>GAZ:00142574</oboInOwl:id>
        <rdfs:label>Otawee Point</rdfs:label>
    </owl:NamedIndividual>
    


    <!-- http://purl.obolibrary.org/obo/GAZ_00142575 -->

    <owl:NamedIndividual rdf:about="http://purl.obolibrary.org/obo/GAZ_00142575">
        <obo:RO_0001025 rdf:resource="http://purl.obolibrary.org/obo/GAZ_00016318"/>
        <obo:IAO_0000115>A lake in the S of Chatham Island.</obo:IAO_0000115>
        <oboInOwl:hasOBONamespace>GAZ</oboInOwl:hasOBONamespace>
        <oboInOwl:id>GAZ:00142575</oboInOwl:id>
        <rdfs:label>Lake Rakeinui</rdfs:label>
    </owl:NamedIndividual>
    


    <!-- http://purl.obolibrary.org/obo/GAZ_00142576 -->

    <owl:NamedIndividual rdf:about="http://purl.obolibrary.org/obo/GAZ_00142576">
        <obo:RO_0001025 rdf:resource="http://purl.obolibrary.org/obo/GAZ_00016318"/>
        <obo:IAO_0000115>A lake in the S of Chatham Island.</obo:IAO_0000115>
        <oboInOwl:hasOBONamespace>GAZ</oboInOwl:hasOBONamespace>
        <oboInOwl:id>GAZ:00142576</oboInOwl:id>
        <rdfs:label>Lake Te Rangatapu</rdfs:label>
    </owl:NamedIndividual>
    


    <!-- http://purl.obolibrary.org/obo/GAZ_00142577 -->

    <owl:NamedIndividual rdf:about="http://purl.obolibrary.org/obo/GAZ_00142577">
        <rdf:type rdf:resource="http://purl.obolibrary.org/obo/ENVO_00000305"/>
        <obo:RO_0001025 rdf:resource="http://purl.obolibrary.org/obo/GAZ_00016318"/>
        <obo:IAO_0000115>A headland into the SW of Te Whanga Lagoon.</obo:IAO_0000115>
        <oboInOwl:hasOBONamespace>GAZ</oboInOwl:hasOBONamespace>
        <oboInOwl:id>GAZ:00142577</oboInOwl:id>
        <rdfs:label>Te Matarae Point</rdfs:label>
    </owl:NamedIndividual>
    


    <!-- http://purl.obolibrary.org/obo/GAZ_00142578 -->

    <owl:NamedIndividual rdf:about="http://purl.obolibrary.org/obo/GAZ_00142578">
        <obo:RO_0001025 rdf:resource="http://purl.obolibrary.org/obo/GAZ_00016318"/>
        <obo:IAO_0000115>The N point of the broad peninsula at Waitangi.</obo:IAO_0000115>
        <oboInOwl:hasOBONamespace>GAZ</oboInOwl:hasOBONamespace>
        <oboInOwl:id>GAZ:00142578</oboInOwl:id>
        <rdfs:label>Point Wedding</rdfs:label>
    </owl:NamedIndividual>
    


    <!-- http://purl.obolibrary.org/obo/GAZ_00142579 -->

    <owl:NamedIndividual rdf:about="http://purl.obolibrary.org/obo/GAZ_00142579">
        <obo:RO_0001025 rdf:resource="http://purl.obolibrary.org/obo/GAZ_00016318"/>
        <obo:IAO_0000115>The NE point of the broad peninsula at Waitangi.</obo:IAO_0000115>
        <oboInOwl:hasOBONamespace>GAZ</oboInOwl:hasOBONamespace>
        <oboInOwl:id>GAZ:00142579</oboInOwl:id>
        <rdfs:label>Point Webb</rdfs:label>
    </owl:NamedIndividual>
    


    <!-- http://purl.obolibrary.org/obo/GAZ_00142580 -->

    <owl:NamedIndividual rdf:about="http://purl.obolibrary.org/obo/GAZ_00142580">
        <obo:RO_0001025 rdf:resource="http://purl.obolibrary.org/obo/GAZ_00016318"/>
        <obo:IAO_0000115>The W point of the broad peninsula at Waitangi.</obo:IAO_0000115>
        <oboInOwl:hasOBONamespace>GAZ</oboInOwl:hasOBONamespace>
        <oboInOwl:id>GAZ:00142580</oboInOwl:id>
        <rdfs:label>Kahunene Point</rdfs:label>
    </owl:NamedIndividual>
    


    <!-- http://purl.obolibrary.org/obo/GAZ_00142581 -->

    <owl:NamedIndividual rdf:about="http://purl.obolibrary.org/obo/GAZ_00142581">
        <obo:RO_0001025 rdf:resource="http://purl.obolibrary.org/obo/GAZ_00016318"/>
        <obo:IAO_0000115>The E point of the broad peninsula at Waitangi.</obo:IAO_0000115>
        <oboInOwl:hasOBONamespace>GAZ</oboInOwl:hasOBONamespace>
        <oboInOwl:id>GAZ:00142581</oboInOwl:id>
        <rdfs:label>Hanson Point</rdfs:label>
    </owl:NamedIndividual>
    


    <!-- http://purl.obolibrary.org/obo/GAZ_00142582 -->

    <owl:NamedIndividual rdf:about="http://purl.obolibrary.org/obo/GAZ_00142582">
        <obo:RO_0001025 rdf:resource="http://purl.obolibrary.org/obo/GAZ_00016318"/>
        <obo:IAO_0000115>A lake between Waitangi (to the W) and Te Whanga Lagoon (to the E).</obo:IAO_0000115>
        <oboInOwl:hasOBONamespace>GAZ</oboInOwl:hasOBONamespace>
        <oboInOwl:id>GAZ:00142582</oboInOwl:id>
        <rdfs:label>Lake Huro</rdfs:label>
    </owl:NamedIndividual>
    


    <!-- http://purl.obolibrary.org/obo/GAZ_00142583 -->

    <owl:NamedIndividual rdf:about="http://purl.obolibrary.org/obo/GAZ_00142583">
        <rdf:type rdf:resource="http://purl.obolibrary.org/obo/ENVO_00000087"/>
        <obo:RO_0001025 rdf:resource="http://purl.obolibrary.org/obo/GAZ_00016318"/>
        <obo:IAO_0000115>A bluff on the coast of Petre Bay.</obo:IAO_0000115>
        <oboInOwl:hasOBONamespace>GAZ</oboInOwl:hasOBONamespace>
        <oboInOwl:id>GAZ:00142583</oboInOwl:id>
        <rdfs:label>Red Bluff</rdfs:label>
    </owl:NamedIndividual>
    


    <!-- http://purl.obolibrary.org/obo/GAZ_00142584 -->

    <owl:NamedIndividual rdf:about="http://purl.obolibrary.org/obo/GAZ_00142584">
        <rdf:type rdf:resource="http://purl.obolibrary.org/obo/ENVO_00000167"/>
        <obo:RO_0001025 rdf:resource="http://purl.obolibrary.org/obo/GAZ_00016318"/>
        <obo:IAO_0000115>A NE point of the broad peninsula at Waitangi, between Point Webb (to the N) and Hanson Point (to the S).</obo:IAO_0000115>
        <oboInOwl:hasOBONamespace>GAZ</oboInOwl:hasOBONamespace>
        <oboInOwl:id>GAZ:00142584</oboInOwl:id>
        <rdfs:label>Ellice Point</rdfs:label>
    </owl:NamedIndividual>
    


    <!-- http://purl.obolibrary.org/obo/GAZ_00142585 -->

    <owl:NamedIndividual rdf:about="http://purl.obolibrary.org/obo/GAZ_00142585">
        <obo:RO_0001025 rdf:resource="http://purl.obolibrary.org/obo/GAZ_00016318"/>
        <obo:IAO_0000115>A short point into the SW of Te Whanga Lagoon, S of Motuhinahina Point.</obo:IAO_0000115>
        <oboInOwl:hasOBONamespace>GAZ</oboInOwl:hasOBONamespace>
        <oboInOwl:id>GAZ:00142585</oboInOwl:id>
        <rdfs:label>Kaiparakau Point</rdfs:label>
    </owl:NamedIndividual>
    


    <!-- http://purl.obolibrary.org/obo/GAZ_00142586 -->

    <owl:NamedIndividual rdf:about="http://purl.obolibrary.org/obo/GAZ_00142586">
        <rdf:type rdf:resource="http://purl.obolibrary.org/obo/ENVO_00000305"/>
        <obo:RO_0001025 rdf:resource="http://purl.obolibrary.org/obo/GAZ_00016318"/>
        <obo:IAO_0000115>A headland into the SW of Te Whanga Lagoon.</obo:IAO_0000115>
        <oboInOwl:hasOBONamespace>GAZ</oboInOwl:hasOBONamespace>
        <oboInOwl:id>GAZ:00142586</oboInOwl:id>
        <rdfs:label>Motuhou Point</rdfs:label>
    </owl:NamedIndividual>
    


    <!-- http://purl.obolibrary.org/obo/GAZ_00142587 -->

    <owl:NamedIndividual rdf:about="http://purl.obolibrary.org/obo/GAZ_00142587">
        <obo:RO_0001025 rdf:resource="http://purl.obolibrary.org/obo/GAZ_00058757"/>
        <obo:IAO_0000115>An island in the SE of Te Whanga Lagoon.</obo:IAO_0000115>
        <oboInOwl:hasOBONamespace>GAZ</oboInOwl:hasOBONamespace>
        <oboInOwl:id>GAZ:00142587</oboInOwl:id>
        <rdfs:label>Waikawa Island</rdfs:label>
    </owl:NamedIndividual>
    


    <!-- http://purl.obolibrary.org/obo/GAZ_00142588 -->

    <owl:NamedIndividual rdf:about="http://purl.obolibrary.org/obo/GAZ_00142588">
        <obo:RO_0001025 rdf:resource="http://purl.obolibrary.org/obo/GAZ_00058757"/>
        <obo:IAO_0000115>A thin island in the SE of Te Whanga Lagoon.</obo:IAO_0000115>
        <oboInOwl:hasOBONamespace>GAZ</oboInOwl:hasOBONamespace>
        <oboInOwl:id>GAZ:00142588</oboInOwl:id>
        <rdfs:label>Moturanganga Island</rdfs:label>
    </owl:NamedIndividual>
    


    <!-- http://purl.obolibrary.org/obo/GAZ_00142589 -->

    <owl:NamedIndividual rdf:about="http://purl.obolibrary.org/obo/GAZ_00142589">
        <obo:RO_0001025 rdf:resource="http://purl.obolibrary.org/obo/GAZ_00058757"/>
        <obo:IAO_0000115>Rocks SE of Motuhinahina Island.</obo:IAO_0000115>
        <oboInOwl:hasOBONamespace>GAZ</oboInOwl:hasOBONamespace>
        <oboInOwl:id>GAZ:00142589</oboInOwl:id>
        <rdfs:label>Limestone Rocks</rdfs:label>
    </owl:NamedIndividual>
    


    <!-- http://purl.obolibrary.org/obo/GAZ_00142590 -->

    <owl:NamedIndividual rdf:about="http://purl.obolibrary.org/obo/GAZ_00142590">
        <obo:RO_0001025 rdf:resource="http://purl.obolibrary.org/obo/GAZ_00058757"/>
        <obo:IAO_0000115>An island in the S of Te Whanga Lagoon.</obo:IAO_0000115>
        <oboInOwl:hasOBONamespace>GAZ</oboInOwl:hasOBONamespace>
        <oboInOwl:id>GAZ:00142590</oboInOwl:id>
        <rdfs:label>Motuhinahina Island</rdfs:label>
    </owl:NamedIndividual>
    


    <!-- http://purl.obolibrary.org/obo/GAZ_00142591 -->

    <owl:NamedIndividual rdf:about="http://purl.obolibrary.org/obo/GAZ_00142591">
        <obo:RO_0001025 rdf:resource="http://purl.obolibrary.org/obo/GAZ_00016318"/>
        <obo:IAO_0000115>A headland pointing SE into the S part of Te Whanga Lagoon.</obo:IAO_0000115>
        <oboInOwl:hasOBONamespace>GAZ</oboInOwl:hasOBONamespace>
        <oboInOwl:id>GAZ:00142591</oboInOwl:id>
        <rdfs:label>Waikato Point</rdfs:label>
    </owl:NamedIndividual>
    


    <!-- http://purl.obolibrary.org/obo/GAZ_00142592 -->

    <owl:NamedIndividual rdf:about="http://purl.obolibrary.org/obo/GAZ_00142592">
        <obo:RO_0001025 rdf:resource="http://purl.obolibrary.org/obo/GAZ_00016318"/>
        <obo:IAO_0000115>A lake to the E of Te Whanga Lagoon.</obo:IAO_0000115>
        <oboInOwl:hasOBONamespace>GAZ</oboInOwl:hasOBONamespace>
        <oboInOwl:id>GAZ:00142592</oboInOwl:id>
        <rdfs:label>Lake Taia</rdfs:label>
    </owl:NamedIndividual>
    


    <!-- http://purl.obolibrary.org/obo/GAZ_00142593 -->

    <owl:NamedIndividual rdf:about="http://purl.obolibrary.org/obo/GAZ_00142593">
        <obo:RO_0001025 rdf:resource="http://purl.obolibrary.org/obo/GAZ_00016318"/>
        <obo:IAO_0000115>A lake to the E of Te Whanga Lagoon.</obo:IAO_0000115>
        <oboInOwl:hasOBONamespace>GAZ</oboInOwl:hasOBONamespace>
        <oboInOwl:id>GAZ:00142593</oboInOwl:id>
        <rdfs:label>Long Pond</rdfs:label>
    </owl:NamedIndividual>
    


    <!-- http://purl.obolibrary.org/obo/GAZ_00142594 -->

    <owl:NamedIndividual rdf:about="http://purl.obolibrary.org/obo/GAZ_00142594">
        <obo:RO_0001025 rdf:resource="http://purl.obolibrary.org/obo/GAZ_00016318"/>
        <obo:IAO_0000115>A lake to the E of Te Whanga Lagoon.</obo:IAO_0000115>
        <oboInOwl:hasOBONamespace>GAZ</oboInOwl:hasOBONamespace>
        <oboInOwl:id>GAZ:00142594</oboInOwl:id>
        <rdfs:label>Lake Kairae</rdfs:label>
    </owl:NamedIndividual>
    


    <!-- http://purl.obolibrary.org/obo/GAZ_00142595 -->

    <owl:NamedIndividual rdf:about="http://purl.obolibrary.org/obo/GAZ_00142595">
        <obo:RO_0001025 rdf:resource="http://purl.obolibrary.org/obo/GAZ_00016318"/>
        <obo:IAO_0000115>The point of a N facing peninsula into the W of Te Whanga Lagoon.</obo:IAO_0000115>
        <oboInOwl:hasOBONamespace>GAZ</oboInOwl:hasOBONamespace>
        <oboInOwl:id>GAZ:00142595</oboInOwl:id>
        <rdfs:label>Kahupiri Point</rdfs:label>
    </owl:NamedIndividual>
    


    <!-- http://purl.obolibrary.org/obo/GAZ_00142596 -->

    <owl:NamedIndividual rdf:about="http://purl.obolibrary.org/obo/GAZ_00142596">
        <obo:RO_0001025 rdf:resource="http://purl.obolibrary.org/obo/GAZ_00016318"/>
        <obo:IAO_0000115>A lake to the E of Te Whanga Lagoon.</obo:IAO_0000115>
        <oboInOwl:hasOBONamespace>GAZ</oboInOwl:hasOBONamespace>
        <oboInOwl:id>GAZ:00142596</oboInOwl:id>
        <rdfs:label>Lake Kaingarahu</rdfs:label>
    </owl:NamedIndividual>
    


    <!-- http://purl.obolibrary.org/obo/GAZ_00142597 -->

    <owl:NamedIndividual rdf:about="http://purl.obolibrary.org/obo/GAZ_00142597">
        <obo:RO_0001025 rdf:resource="http://purl.obolibrary.org/obo/GAZ_00016318"/>
        <obo:IAO_0000115>A lake W of Te Whanga Lagoon, behind Long Beach.</obo:IAO_0000115>
        <oboInOwl:hasOBONamespace>GAZ</oboInOwl:hasOBONamespace>
        <oboInOwl:id>GAZ:00142597</oboInOwl:id>
        <rdfs:label>Lake Marakapia</rdfs:label>
    </owl:NamedIndividual>
    


    <!-- http://purl.obolibrary.org/obo/GAZ_00142598 -->

    <owl:NamedIndividual rdf:about="http://purl.obolibrary.org/obo/GAZ_00142598">
        <obo:RO_0001025 rdf:resource="http://purl.obolibrary.org/obo/GAZ_00016318"/>
        <obo:IAO_0000115>A lake W of Te Whanga Lagoon, behind Long Beach.</obo:IAO_0000115>
        <oboInOwl:hasOBONamespace>GAZ</oboInOwl:hasOBONamespace>
        <oboInOwl:id>GAZ:00142598</oboInOwl:id>
        <rdfs:label>Te Roto</rdfs:label>
    </owl:NamedIndividual>
    


    <!-- http://purl.obolibrary.org/obo/GAZ_00142599 -->

    <owl:NamedIndividual rdf:about="http://purl.obolibrary.org/obo/GAZ_00142599">
        <obo:RO_0001025 rdf:resource="http://purl.obolibrary.org/obo/GAZ_00016318"/>
        <obo:IAO_0000115>The point of a peninsula pointing S into the N of Petre Bay.</obo:IAO_0000115>
        <oboInOwl:hasOBONamespace>GAZ</oboInOwl:hasOBONamespace>
        <oboInOwl:id>GAZ:00142599</oboInOwl:id>
        <rdfs:label>Napper Point</rdfs:label>
    </owl:NamedIndividual>
    


    <!-- http://purl.obolibrary.org/obo/GAZ_00142600 -->

    <owl:NamedIndividual rdf:about="http://purl.obolibrary.org/obo/GAZ_00142600">
        <obo:RO_0001025 rdf:resource="http://purl.obolibrary.org/obo/GAZ_00016318"/>
        <obo:IAO_0000115>A headland pointing E into the S part of Te Whanga Lagoon.</obo:IAO_0000115>
        <oboInOwl:hasOBONamespace>GAZ</oboInOwl:hasOBONamespace>
        <oboInOwl:id>GAZ:00142600</oboInOwl:id>
        <rdfs:label>Moutapu Point</rdfs:label>
    </owl:NamedIndividual>
    


    <!-- http://purl.obolibrary.org/obo/GAZ_00142601 -->

    <owl:NamedIndividual rdf:about="http://purl.obolibrary.org/obo/GAZ_00142601">
        <obo:RO_0001025 rdf:resource="http://purl.obolibrary.org/obo/GAZ_00016318"/>
        <obo:IAO_0000115>A lake W of Te Whanga Lagoon, behind Long Beach.</obo:IAO_0000115>
        <oboInOwl:hasOBONamespace>GAZ</oboInOwl:hasOBONamespace>
        <oboInOwl:id>GAZ:00142601</oboInOwl:id>
        <rdfs:label>Lake Rotoparaoa</rdfs:label>
    </owl:NamedIndividual>
    


    <!-- http://purl.obolibrary.org/obo/GAZ_00142602 -->

    <owl:NamedIndividual rdf:about="http://purl.obolibrary.org/obo/GAZ_00142602">
        <obo:RO_0001025 rdf:resource="http://purl.obolibrary.org/obo/GAZ_00016318"/>
        <obo:IAO_0000115>A lake W of Te Whanga Lagoon, behind Long Beach.</obo:IAO_0000115>
        <oboInOwl:hasOBONamespace>GAZ</oboInOwl:hasOBONamespace>
        <oboInOwl:id>GAZ:00142602</oboInOwl:id>
        <rdfs:label>Tennants Lake</rdfs:label>
    </owl:NamedIndividual>
    


    <!-- http://purl.obolibrary.org/obo/GAZ_00142603 -->

    <owl:NamedIndividual rdf:about="http://purl.obolibrary.org/obo/GAZ_00142603">
        <obo:RO_0001025 rdf:resource="http://purl.obolibrary.org/obo/GAZ_00058757"/>
        <obo:IAO_0000115>One of a group of 5 islands N of Kahupiri Point.</obo:IAO_0000115>
        <oboInOwl:hasOBONamespace>GAZ</oboInOwl:hasOBONamespace>
        <oboInOwl:id>GAZ:00142603</oboInOwl:id>
        <rdfs:label>Titihaukai Island</rdfs:label>
    </owl:NamedIndividual>
    


    <!-- http://purl.obolibrary.org/obo/GAZ_00142604 -->

    <owl:NamedIndividual rdf:about="http://purl.obolibrary.org/obo/GAZ_00142604">
        <obo:RO_0001025 rdf:resource="http://purl.obolibrary.org/obo/GAZ_00058757"/>
        <obo:IAO_0000115>A bay on the NW of the southern part of Te Whanga Lagoon, between Waikato Point and Moutapu Point.</obo:IAO_0000115>
        <oboInOwl:hasOBONamespace>GAZ</oboInOwl:hasOBONamespace>
        <oboInOwl:id>GAZ:00142604</oboInOwl:id>
        <rdfs:label>Waikato Bay</rdfs:label>
    </owl:NamedIndividual>
    


    <!-- http://purl.obolibrary.org/obo/GAZ_00142605 -->

    <owl:NamedIndividual rdf:about="http://purl.obolibrary.org/obo/GAZ_00142605">
        <obo:RO_0001025 rdf:resource="http://purl.obolibrary.org/obo/GAZ_00146862"/>
        <obo:IAO_0000115>A reef in the N part of Petre Bay.</obo:IAO_0000115>
        <oboInOwl:hasOBONamespace>GAZ</oboInOwl:hasOBONamespace>
        <oboInOwl:id>GAZ:00142605</oboInOwl:id>
        <rdfs:label>Island Reef</rdfs:label>
    </owl:NamedIndividual>
    


    <!-- http://purl.obolibrary.org/obo/GAZ_00142606 -->

    <owl:NamedIndividual rdf:about="http://purl.obolibrary.org/obo/GAZ_00142606">
        <obo:RO_0001025 rdf:resource="http://purl.obolibrary.org/obo/GAZ_00016318"/>
        <obo:IAO_0000115>The point of a broad peninsula in the N of Petre Bay.</obo:IAO_0000115>
        <oboInOwl:hasOBONamespace>GAZ</oboInOwl:hasOBONamespace>
        <oboInOwl:id>GAZ:00142606</oboInOwl:id>
        <rdfs:label>Point Dorset</rdfs:label>
    </owl:NamedIndividual>
    


    <!-- http://purl.obolibrary.org/obo/GAZ_00142607 -->

    <owl:NamedIndividual rdf:about="http://purl.obolibrary.org/obo/GAZ_00142607">
        <obo:RO_0001025 rdf:resource="http://purl.obolibrary.org/obo/GAZ_00016318"/>
        <obo:IAO_0000115>A blunt point on the NW of the western peninusla of Chatham Island.</obo:IAO_0000115>
        <oboInOwl:hasOBONamespace>GAZ</oboInOwl:hasOBONamespace>
        <oboInOwl:id>GAZ:00142607</oboInOwl:id>
        <rdfs:label>Point Alison</rdfs:label>
    </owl:NamedIndividual>
    


    <!-- http://purl.obolibrary.org/obo/GAZ_00142608 -->

    <owl:NamedIndividual rdf:about="http://purl.obolibrary.org/obo/GAZ_00142608">
        <obo:RO_0001025 rdf:resource="http://purl.obolibrary.org/obo/GAZ_00016318"/>
        <obo:IAO_0000115>A lake in the W of the northwestern peninsula of Chatham Island.</obo:IAO_0000115>
        <oboInOwl:hasOBONamespace>GAZ</oboInOwl:hasOBONamespace>
        <oboInOwl:id>GAZ:00142608</oboInOwl:id>
        <rdfs:label>Lake Rotokawau</rdfs:label>
    </owl:NamedIndividual>
    


    <!-- http://purl.obolibrary.org/obo/GAZ_00142609 -->

    <owl:NamedIndividual rdf:about="http://purl.obolibrary.org/obo/GAZ_00142609">
        <rdf:type rdf:resource="http://purl.obolibrary.org/obo/ENVO_00000305"/>
        <obo:RO_0001025 rdf:resource="http://purl.obolibrary.org/obo/GAZ_00016318"/>
        <obo:IAO_0000115>A headland at the S of the northwestern peninsula of Chatham Island.</obo:IAO_0000115>
        <oboInOwl:hasOBONamespace>GAZ</oboInOwl:hasOBONamespace>
        <oboInOwl:id>GAZ:00142609</oboInOwl:id>
        <rdfs:label>Point Somes</rdfs:label>
    </owl:NamedIndividual>
    


    <!-- http://purl.obolibrary.org/obo/GAZ_00142610 -->

    <owl:NamedIndividual rdf:about="http://purl.obolibrary.org/obo/GAZ_00142610">
        <obo:RO_0001025 rdf:resource="http://purl.obolibrary.org/obo/GAZ_00016318"/>
        <obo:IAO_0000115>The W point of Chatham Island.</obo:IAO_0000115>
        <oboInOwl:hasOBONamespace>GAZ</oboInOwl:hasOBONamespace>
        <oboInOwl:id>GAZ:00142610</oboInOwl:id>
        <rdfs:label>Te Raki Point</rdfs:label>
    </owl:NamedIndividual>
    


    <!-- http://purl.obolibrary.org/obo/GAZ_00142611 -->

    <owl:NamedIndividual rdf:about="http://purl.obolibrary.org/obo/GAZ_00142611">
        <obo:RO_0001025 rdf:resource="http://purl.obolibrary.org/obo/GAZ_00016318"/>
        <obo:IAO_0000115>A lake in the W of the northwestern peninsula of Chatham Island.</obo:IAO_0000115>
        <oboInOwl:hasOBONamespace>GAZ</oboInOwl:hasOBONamespace>
        <oboInOwl:id>GAZ:00142611</oboInOwl:id>
        <rdfs:label>Lake Rotoeka</rdfs:label>
    </owl:NamedIndividual>
    


    <!-- http://purl.obolibrary.org/obo/GAZ_00142612 -->

    <owl:NamedIndividual rdf:about="http://purl.obolibrary.org/obo/GAZ_00142612">
        <obo:RO_0001025 rdf:resource="http://purl.obolibrary.org/obo/GAZ_00016318"/>
        <obo:IAO_0000115>The point of a peninsula that, on the W, divides Te Whanga Lagoon into N and S parts.</obo:IAO_0000115>
        <oboInOwl:hasOBONamespace>GAZ</oboInOwl:hasOBONamespace>
        <oboInOwl:id>GAZ:00142612</oboInOwl:id>
        <rdfs:label>Karewa Point</rdfs:label>
    </owl:NamedIndividual>
    


    <!-- http://purl.obolibrary.org/obo/GAZ_00142613 -->

    <owl:NamedIndividual rdf:about="http://purl.obolibrary.org/obo/GAZ_00142613">
        <obo:RO_0001025 rdf:resource="http://purl.obolibrary.org/obo/GAZ_00016318"/>
        <obo:IAO_0000115>A river discharging to the S of Te Whanga Lagoon.</obo:IAO_0000115>
        <oboInOwl:hasOBONamespace>GAZ</oboInOwl:hasOBONamespace>
        <oboInOwl:id>GAZ:00142613</oboInOwl:id>
        <rdfs:label>Te Awainanga River</rdfs:label>
    </owl:NamedIndividual>
    


    <!-- http://purl.obolibrary.org/obo/GAZ_00142614 -->

    <owl:NamedIndividual rdf:about="http://purl.obolibrary.org/obo/GAZ_00142614">
        <obo:RO_0001025 rdf:resource="http://purl.obolibrary.org/obo/GAZ_00016318"/>
        <obo:IAO_0000115>The most E point of the southern part of Chatham Island, at the S of Hanson Bay.</obo:IAO_0000115>
        <oboInOwl:hasOBONamespace>GAZ</oboInOwl:hasOBONamespace>
        <oboInOwl:id>GAZ:00142614</oboInOwl:id>
        <rdfs:label>Manukau Point</rdfs:label>
    </owl:NamedIndividual>
    


    <!-- http://purl.obolibrary.org/obo/GAZ_00142615 -->

    <owl:NamedIndividual rdf:about="http://purl.obolibrary.org/obo/GAZ_00142615">
        <obo:RO_0001025 rdf:resource="http://purl.obolibrary.org/obo/GAZ_00047005"/>
        <obo:IAO_0000115>Small islands off the NW of Stewart Island.</obo:IAO_0000115>
        <oboInOwl:hasOBONamespace>GAZ</oboInOwl:hasOBONamespace>
        <oboInOwl:id>GAZ:00142615</oboInOwl:id>
        <rdfs:label>Bishop and Clerke Islands</rdfs:label>
    </owl:NamedIndividual>
    


    <!-- http://purl.obolibrary.org/obo/GAZ_00142616 -->

    <owl:NamedIndividual rdf:about="http://purl.obolibrary.org/obo/GAZ_00142616">
        <rdf:type rdf:resource="http://purl.obolibrary.org/obo/ENVO_00000305"/>
        <obo:RO_0001025 rdf:resource="http://purl.obolibrary.org/obo/GAZ_00016318"/>
        <obo:IAO_0000115>A NW cape of Chatham Island.</obo:IAO_0000115>
        <oboInOwl:hasOBONamespace>GAZ</oboInOwl:hasOBONamespace>
        <oboInOwl:id>GAZ:00142616</oboInOwl:id>
        <rdfs:label>Cape Pattisson</rdfs:label>
    </owl:NamedIndividual>
    


    <!-- http://purl.obolibrary.org/obo/GAZ_00142617 -->

    <owl:NamedIndividual rdf:about="http://purl.obolibrary.org/obo/GAZ_00142617">
        <obo:RO_0001025 rdf:resource="http://purl.obolibrary.org/obo/GAZ_00007126"/>
        <obo:IAO_0000115>A reef SW of Point Somes.</obo:IAO_0000115>
        <oboInOwl:hasOBONamespace>GAZ</oboInOwl:hasOBONamespace>
        <oboInOwl:id>GAZ:00142617</oboInOwl:id>
        <rdfs:label>Western Reef</rdfs:label>
    </owl:NamedIndividual>
    


    <!-- http://purl.obolibrary.org/obo/GAZ_00142622 -->

    <owl:NamedIndividual rdf:about="http://purl.obolibrary.org/obo/GAZ_00142622">
        <obo:RO_0001025 rdf:resource="http://purl.obolibrary.org/obo/GAZ_00007126"/>
        <obo:IAO_0000115>A reef off the NW of Chatham Island, to the W of the broad peninsula capped by Cape Pattisson.</obo:IAO_0000115>
        <oboInOwl:hasOBONamespace>GAZ</oboInOwl:hasOBONamespace>
        <oboInOwl:id>GAZ:00142622</oboInOwl:id>
        <rdfs:label>Tapuangi-Monau Reef</rdfs:label>
    </owl:NamedIndividual>
    


    <!-- http://purl.obolibrary.org/obo/GAZ_00142623 -->

    <owl:NamedIndividual rdf:about="http://purl.obolibrary.org/obo/GAZ_00142623">
        <obo:RO_0001025 rdf:resource="http://purl.obolibrary.org/obo/GAZ_00016318"/>
        <obo:IAO_0000115>A lake in the area between the N of te Whanga Lagoon and the N coast of Chatham Island.</obo:IAO_0000115>
        <oboInOwl:hasOBONamespace>GAZ</oboInOwl:hasOBONamespace>
        <oboInOwl:id>GAZ:00142623</oboInOwl:id>
        <rdfs:label>Pakauwera Pond</rdfs:label>
    </owl:NamedIndividual>
    


    <!-- http://purl.obolibrary.org/obo/GAZ_00142624 -->

    <owl:NamedIndividual rdf:about="http://purl.obolibrary.org/obo/GAZ_00142624">
        <rdf:type rdf:resource="http://purl.obolibrary.org/obo/ENVO_00000305"/>
        <obo:RO_0001025 rdf:resource="http://purl.obolibrary.org/obo/GAZ_00016318"/>
        <obo:IAO_0000115>A headland into the NW of Te Whanga Lagoon.</obo:IAO_0000115>
        <oboInOwl:hasOBONamespace>GAZ</oboInOwl:hasOBONamespace>
        <oboInOwl:id>GAZ:00142624</oboInOwl:id>
        <rdfs:label>Cattle Point</rdfs:label>
    </owl:NamedIndividual>
    


    <!-- http://purl.obolibrary.org/obo/GAZ_00142625 -->

    <owl:NamedIndividual rdf:about="http://purl.obolibrary.org/obo/GAZ_00142625">
        <rdf:type rdf:resource="http://purl.obolibrary.org/obo/ENVO_00000305"/>
        <obo:RO_0001025 rdf:resource="http://purl.obolibrary.org/obo/GAZ_00016318"/>
        <obo:IAO_0000115>A headland into the NW of Te Whanga Lagoon.</obo:IAO_0000115>
        <oboInOwl:hasOBONamespace>GAZ</oboInOwl:hasOBONamespace>
        <oboInOwl:id>GAZ:00142625</oboInOwl:id>
        <rdfs:label>Mihitoroa Point</rdfs:label>
    </owl:NamedIndividual>
    


    <!-- http://purl.obolibrary.org/obo/GAZ_00142626 -->

    <owl:NamedIndividual rdf:about="http://purl.obolibrary.org/obo/GAZ_00142626">
        <obo:RO_0001025 rdf:resource="http://purl.obolibrary.org/obo/GAZ_00016318"/>
        <obo:IAO_0000115>A lake in the area between the N of te Whanga Lagoon and the N coast of Chatham Island.</obo:IAO_0000115>
        <oboInOwl:hasOBONamespace>GAZ</oboInOwl:hasOBONamespace>
        <oboInOwl:id>GAZ:00142626</oboInOwl:id>
        <rdfs:label>Lake Wharo</rdfs:label>
    </owl:NamedIndividual>
    


    <!-- http://purl.obolibrary.org/obo/GAZ_00142627 -->

    <owl:NamedIndividual rdf:about="http://purl.obolibrary.org/obo/GAZ_00142627">
        <rdf:type rdf:resource="http://purl.obolibrary.org/obo/ENVO_00000305"/>
        <obo:RO_0001025 rdf:resource="http://purl.obolibrary.org/obo/GAZ_00016318"/>
        <obo:IAO_0000115>A headland into the NW of Te Whanga Lagoon.</obo:IAO_0000115>
        <oboInOwl:hasOBONamespace>GAZ</oboInOwl:hasOBONamespace>
        <oboInOwl:id>GAZ:00142627</oboInOwl:id>
        <rdfs:label>Cemetery Point</rdfs:label>
    </owl:NamedIndividual>
    


    <!-- http://purl.obolibrary.org/obo/GAZ_00142628 -->

    <owl:NamedIndividual rdf:about="http://purl.obolibrary.org/obo/GAZ_00142628">
        <obo:RO_0001025 rdf:resource="http://purl.obolibrary.org/obo/GAZ_00058757"/>
        <obo:IAO_0000115>An island in the NW of Te Whanga Lagoon.</obo:IAO_0000115>
        <oboInOwl:hasOBONamespace>GAZ</oboInOwl:hasOBONamespace>
        <oboInOwl:id>GAZ:00142628</oboInOwl:id>
        <rdfs:label>Moropunga Island</rdfs:label>
    </owl:NamedIndividual>
    


    <!-- http://purl.obolibrary.org/obo/GAZ_00142629 -->

    <owl:NamedIndividual rdf:about="http://purl.obolibrary.org/obo/GAZ_00142629">
        <obo:RO_0001025 rdf:resource="http://purl.obolibrary.org/obo/GAZ_00016318"/>
        <obo:IAO_0000115>A blunt point on the N of Chatham Island.</obo:IAO_0000115>
        <oboInOwl:hasOBONamespace>GAZ</oboInOwl:hasOBONamespace>
        <oboInOwl:id>GAZ:00142629</oboInOwl:id>
        <rdfs:label>Ocean Mail Point</rdfs:label>
    </owl:NamedIndividual>
    


    <!-- http://purl.obolibrary.org/obo/GAZ_00142630 -->

    <owl:NamedIndividual rdf:about="http://purl.obolibrary.org/obo/GAZ_00142630">
        <obo:RO_0001025 rdf:resource="http://purl.obolibrary.org/obo/GAZ_00016318"/>
        <obo:IAO_0000115>A lake in the N of Chatham Island, SE of Lake Pateriki.</obo:IAO_0000115>
        <oboInOwl:hasOBONamespace>GAZ</oboInOwl:hasOBONamespace>
        <oboInOwl:id>GAZ:00142630</oboInOwl:id>
        <rdfs:label>Lake Rotorua</rdfs:label>
    </owl:NamedIndividual>
    


    <!-- http://purl.obolibrary.org/obo/GAZ_00142631 -->

    <owl:NamedIndividual rdf:about="http://purl.obolibrary.org/obo/GAZ_00142631">
        <obo:RO_0001025 rdf:resource="http://purl.obolibrary.org/obo/GAZ_00016318"/>
        <obo:IAO_0000115>A lake in the N of Chatham Island, to the W of Lake Rangitai.</obo:IAO_0000115>
        <oboInOwl:hasOBONamespace>GAZ</oboInOwl:hasOBONamespace>
        <oboInOwl:id>GAZ:00142631</oboInOwl:id>
        <rdfs:label>Lake Kaimoumi</rdfs:label>
    </owl:NamedIndividual>
    


    <!-- http://purl.obolibrary.org/obo/GAZ_00142632 -->

    <owl:NamedIndividual rdf:about="http://purl.obolibrary.org/obo/GAZ_00142632">
        <obo:RO_0001025 rdf:resource="http://purl.obolibrary.org/obo/GAZ_00016318"/>
        <obo:IAO_0000115>A lake in the N of Chatham Island.</obo:IAO_0000115>
        <oboInOwl:hasOBONamespace>GAZ</oboInOwl:hasOBONamespace>
        <oboInOwl:id>GAZ:00142632</oboInOwl:id>
        <rdfs:label>Lake Rangitai</rdfs:label>
    </owl:NamedIndividual>
    


    <!-- http://purl.obolibrary.org/obo/GAZ_00142633 -->

    <owl:NamedIndividual rdf:about="http://purl.obolibrary.org/obo/GAZ_00142633">
        <obo:RO_0001025 rdf:resource="http://purl.obolibrary.org/obo/GAZ_00016318"/>
        <obo:IAO_0000115>A lake in the N of Chatham Island, E of Lake Rangitai.</obo:IAO_0000115>
        <oboInOwl:hasOBONamespace>GAZ</oboInOwl:hasOBONamespace>
        <oboInOwl:id>GAZ:00142633</oboInOwl:id>
        <rdfs:label>Lake Pateriki</rdfs:label>
    </owl:NamedIndividual>
    


    <!-- http://purl.obolibrary.org/obo/GAZ_00142634 -->

    <owl:NamedIndividual rdf:about="http://purl.obolibrary.org/obo/GAZ_00142634">
        <obo:RO_0001025 rdf:resource="http://purl.obolibrary.org/obo/GAZ_00007126"/>
        <obo:IAO_0000115>A reef off the N coast of Chatham Island, N of Ocean Mail Point.</obo:IAO_0000115>
        <oboInOwl:hasOBONamespace>GAZ</oboInOwl:hasOBONamespace>
        <oboInOwl:id>GAZ:00142634</oboInOwl:id>
        <rdfs:label>French Reef</rdfs:label>
    </owl:NamedIndividual>
    


    <!-- http://purl.obolibrary.org/obo/GAZ_00142635 -->

    <owl:NamedIndividual rdf:about="http://purl.obolibrary.org/obo/GAZ_00142635">
        <obo:RO_0001025 rdf:resource="http://purl.obolibrary.org/obo/GAZ_00016318"/>
        <obo:IAO_0000115>The point of the S peninsula in the NE of Chatham Island.</obo:IAO_0000115>
        <oboInOwl:hasOBONamespace>GAZ</oboInOwl:hasOBONamespace>
        <oboInOwl:id>GAZ:00142635</oboInOwl:id>
        <rdfs:label>Owaka Point</rdfs:label>
    </owl:NamedIndividual>
    


    <!-- http://purl.obolibrary.org/obo/GAZ_00142636 -->

    <owl:NamedIndividual rdf:about="http://purl.obolibrary.org/obo/GAZ_00142636">
        <obo:RO_0001025 rdf:resource="http://purl.obolibrary.org/obo/GAZ_00016318"/>
        <obo:IAO_0000115>A lake on the NE peninsula of Chatham Island.</obo:IAO_0000115>
        <oboInOwl:hasOBONamespace>GAZ</oboInOwl:hasOBONamespace>
        <oboInOwl:id>GAZ:00142636</oboInOwl:id>
        <rdfs:label>Lake Te Wapu</rdfs:label>
    </owl:NamedIndividual>
    


    <!-- http://purl.obolibrary.org/obo/GAZ_00142637 -->

    <owl:NamedIndividual rdf:about="http://purl.obolibrary.org/obo/GAZ_00142637">
        <obo:RO_0001025 rdf:resource="http://purl.obolibrary.org/obo/GAZ_00016318"/>
        <obo:IAO_0000115>A small lake on the NE peninsula of Chatham Island.</obo:IAO_0000115>
        <oboInOwl:hasOBONamespace>GAZ</oboInOwl:hasOBONamespace>
        <oboInOwl:id>GAZ:00142637</oboInOwl:id>
        <rdfs:label>Lake Omutu</rdfs:label>
    </owl:NamedIndividual>
    


    <!-- http://purl.obolibrary.org/obo/GAZ_00142638 -->

    <owl:NamedIndividual rdf:about="http://purl.obolibrary.org/obo/GAZ_00142638">
        <obo:RO_0001025 rdf:resource="http://purl.obolibrary.org/obo/GAZ_00016318"/>
        <obo:IAO_0000115>The NE point of Chatham Island.</obo:IAO_0000115>
        <oboInOwl:hasOBONamespace>GAZ</oboInOwl:hasOBONamespace>
        <oboInOwl:id>GAZ:00142638</oboInOwl:id>
        <rdfs:label>Point Munning</rdfs:label>
    </owl:NamedIndividual>
    


    <!-- http://purl.obolibrary.org/obo/GAZ_00142639 -->

    <owl:NamedIndividual rdf:about="http://purl.obolibrary.org/obo/GAZ_00142639">
        <obo:RO_0001025 rdf:resource="http://purl.obolibrary.org/obo/GAZ_00007126"/>
        <obo:IAO_0000115>A reef to the W of Okawa Point in the NE of Chatham Island.</obo:IAO_0000115>
        <oboInOwl:hasOBONamespace>GAZ</oboInOwl:hasOBONamespace>
        <oboInOwl:id>GAZ:00142639</oboInOwl:id>
        <rdfs:label>Manapo Reef</rdfs:label>
    </owl:NamedIndividual>
    


    <!-- http://purl.obolibrary.org/obo/GAZ_00142640 -->

    <owl:NamedIndividual rdf:about="http://purl.obolibrary.org/obo/GAZ_00142640">
        <obo:RO_0001025 rdf:resource="http://purl.obolibrary.org/obo/GAZ_00007126"/>
        <obo:IAO_0000115>An in shore rock on the N coast to the NE peninsula of Chatham Island.</obo:IAO_0000115>
        <oboInOwl:hasOBONamespace>GAZ</oboInOwl:hasOBONamespace>
        <oboInOwl:id>GAZ:00142640</oboInOwl:id>
        <rdfs:label>Omatuku Rock</rdfs:label>
    </owl:NamedIndividual>
    


    <!-- http://purl.obolibrary.org/obo/GAZ_00142641 -->

    <owl:NamedIndividual rdf:about="http://purl.obolibrary.org/obo/GAZ_00142641">
        <obo:RO_0001025 rdf:resource="http://purl.obolibrary.org/obo/GAZ_00007126"/>
        <obo:IAO_0000115>A reef in the broad bay NE of Okawa Point in NE Chatham Island.</obo:IAO_0000115>
        <oboInOwl:hasOBONamespace>GAZ</oboInOwl:hasOBONamespace>
        <oboInOwl:id>GAZ:00142641</oboInOwl:id>
        <rdfs:label>Blind Reef</rdfs:label>
    </owl:NamedIndividual>
    


    <!-- http://purl.obolibrary.org/obo/GAZ_00142642 -->

    <owl:NamedIndividual rdf:about="http://purl.obolibrary.org/obo/GAZ_00142642">
        <obo:RO_0001025 rdf:resource="http://purl.obolibrary.org/obo/GAZ_00007126"/>
        <obo:IAO_0000115>An island E of the NE peninsula of Chatham Island.</obo:IAO_0000115>
        <oboInOwl:hasOBONamespace>GAZ</oboInOwl:hasOBONamespace>
        <oboInOwl:id>GAZ:00142642</oboInOwl:id>
        <rdfs:label>Te Whakuru Island</rdfs:label>
    </owl:NamedIndividual>
    


    <!-- http://purl.obolibrary.org/obo/GAZ_00142643 -->

    <owl:NamedIndividual rdf:about="http://purl.obolibrary.org/obo/GAZ_00142643">
        <obo:RO_0001025 rdf:resource="http://purl.obolibrary.org/obo/GAZ_00007126"/>
        <obo:IAO_0000115>A small in shore island off the NW coast of Chatham Island between Cape Young and Okahu Point.</obo:IAO_0000115>
        <oboInOwl:hasOBONamespace>GAZ</oboInOwl:hasOBONamespace>
        <oboInOwl:id>GAZ:00142643</oboInOwl:id>
        <rdfs:label>Te Awanui island</rdfs:label>
    </owl:NamedIndividual>
    


    <!-- http://purl.obolibrary.org/obo/GAZ_00142644 -->

    <owl:NamedIndividual rdf:about="http://purl.obolibrary.org/obo/GAZ_00142644">
        <obo:RO_0001025 rdf:resource="http://purl.obolibrary.org/obo/GAZ_00016318"/>
        <obo:IAO_0000115>A shallow point on the NW coast of Chatham Island.</obo:IAO_0000115>
        <oboInOwl:hasOBONamespace>GAZ</oboInOwl:hasOBONamespace>
        <oboInOwl:id>GAZ:00142644</oboInOwl:id>
        <rdfs:label>Okahu Point</rdfs:label>
    </owl:NamedIndividual>
    


    <!-- http://purl.obolibrary.org/obo/GAZ_00142645 -->

    <owl:NamedIndividual rdf:about="http://purl.obolibrary.org/obo/GAZ_00142645">
        <obo:RO_0001025 rdf:resource="http://purl.obolibrary.org/obo/GAZ_00016318"/>
        <obo:IAO_0000115>The N peninsula of Chatham Island.</obo:IAO_0000115>
        <oboInOwl:hasOBONamespace>GAZ</oboInOwl:hasOBONamespace>
        <oboInOwl:id>GAZ:00142645</oboInOwl:id>
        <rdfs:label>Cape Young</rdfs:label>
    </owl:NamedIndividual>
    


    <!-- http://purl.obolibrary.org/obo/GAZ_00142646 -->

    <owl:NamedIndividual rdf:about="http://purl.obolibrary.org/obo/GAZ_00142646">
        <obo:RO_0001025 rdf:resource="http://purl.obolibrary.org/obo/GAZ_00016318"/>
        <obo:IAO_0000115>A lake in the NW of Chatham Island, S of Cape Young.</obo:IAO_0000115>
        <oboInOwl:hasOBONamespace>GAZ</oboInOwl:hasOBONamespace>
        <oboInOwl:id>GAZ:00142646</oboInOwl:id>
        <rdfs:label>Lake Waikauia</rdfs:label>
    </owl:NamedIndividual>
    


    <!-- http://purl.obolibrary.org/obo/GAZ_00142647 -->

    <owl:NamedIndividual rdf:about="http://purl.obolibrary.org/obo/GAZ_00142647">
        <obo:RO_0001025 rdf:resource="http://purl.obolibrary.org/obo/GAZ_00047005"/>
        <obo:IAO_0000115>Small islands off the NW of Stewart Island.</obo:IAO_0000115>
        <oboInOwl:hasOBONamespace>GAZ</oboInOwl:hasOBONamespace>
        <oboInOwl:id>GAZ:00142647</oboInOwl:id>
        <rdfs:label>Rugged Islands</rdfs:label>
    </owl:NamedIndividual>
    


    <!-- http://purl.obolibrary.org/obo/GAZ_00142651 -->

    <owl:NamedIndividual rdf:about="http://purl.obolibrary.org/obo/GAZ_00142651">
        <obo:RO_0001025 rdf:resource="http://purl.obolibrary.org/obo/GAZ_00004774"/>
        <obo:IAO_0000115>A N pointing peninsula marking the S entrance of Paterson Inlet.</obo:IAO_0000115>
        <oboInOwl:hasOBONamespace>GAZ</oboInOwl:hasOBONamespace>
        <oboInOwl:id>GAZ:00142651</oboInOwl:id>
        <rdfs:label>The Neck</rdfs:label>
    </owl:NamedIndividual>
    


    <!-- http://purl.obolibrary.org/obo/GAZ_00142652 -->

    <owl:NamedIndividual rdf:about="http://purl.obolibrary.org/obo/GAZ_00142652">
        <obo:RO_0001025 rdf:resource="http://purl.obolibrary.org/obo/GAZ_00004774"/>
        <obo:IAO_0000115>The SW cape of Stewart Island, to the W of South Cape.</obo:IAO_0000115>
        <oboInOwl:hasOBONamespace>GAZ</oboInOwl:hasOBONamespace>
        <oboInOwl:id>GAZ:00142652</oboInOwl:id>
        <rdfs:label>South West Cape</rdfs:label>
    </owl:NamedIndividual>
    


    <!-- http://purl.obolibrary.org/obo/GAZ_00142653 -->

    <owl:NamedIndividual rdf:about="http://purl.obolibrary.org/obo/GAZ_00142653">
        <obo:RO_0001025 rdf:resource="http://purl.obolibrary.org/obo/GAZ_00004774"/>
        <obo:IAO_0000115>The SE point of Stewart Island.</obo:IAO_0000115>
        <oboInOwl:hasOBONamespace>GAZ</oboInOwl:hasOBONamespace>
        <oboInOwl:id>GAZ:00142653</oboInOwl:id>
        <rdfs:label>Shelter Point</rdfs:label>
    </owl:NamedIndividual>
    


    <!-- http://purl.obolibrary.org/obo/GAZ_00142654 -->

    <owl:NamedIndividual rdf:about="http://purl.obolibrary.org/obo/GAZ_00142654">
        <rdf:type rdf:resource="http://purl.obolibrary.org/obo/ENVO_00000305"/>
        <obo:RO_0001025 rdf:resource="http://purl.obolibrary.org/obo/GAZ_00004774"/>
        <obo:IAO_0000115>A cape on the SW of Stewart Island, to the E of South West Cape.</obo:IAO_0000115>
        <oboInOwl:hasOBONamespace>GAZ</oboInOwl:hasOBONamespace>
        <oboInOwl:id>GAZ:00142654</oboInOwl:id>
        <rdfs:label>South Cape</rdfs:label>
    </owl:NamedIndividual>
    


    <!-- http://purl.obolibrary.org/obo/GAZ_00142662 -->

    <owl:NamedIndividual rdf:about="http://purl.obolibrary.org/obo/GAZ_00142662">
        <obo:RO_0001025 rdf:resource="http://purl.obolibrary.org/obo/GAZ_00047005"/>
        <obo:IAO_0000115>A small island E of Ruapuke Island.</obo:IAO_0000115>
        <oboInOwl:hasOBONamespace>GAZ</oboInOwl:hasOBONamespace>
        <oboInOwl:id>GAZ:00142662</oboInOwl:id>
        <rdfs:label>Green Island</rdfs:label>
    </owl:NamedIndividual>
    


    <!-- http://purl.obolibrary.org/obo/GAZ_00142663 -->

    <owl:NamedIndividual rdf:about="http://purl.obolibrary.org/obo/GAZ_00142663">
        <obo:RO_0001025 rdf:resource="http://purl.obolibrary.org/obo/GAZ_00047005"/>
        <obo:IAO_0000115>Islands to the S of Ruapuke Island.</obo:IAO_0000115>
        <oboInOwl:hasOBONamespace>GAZ</oboInOwl:hasOBONamespace>
        <oboInOwl:id>GAZ:00142663</oboInOwl:id>
        <rdfs:label>Hazelburgh Group</rdfs:label>
    </owl:NamedIndividual>
    


    <!-- http://purl.obolibrary.org/obo/GAZ_00142664 -->

    <owl:NamedIndividual rdf:about="http://purl.obolibrary.org/obo/GAZ_00142664">
        <obo:RO_0001025 rdf:resource="http://purl.obolibrary.org/obo/GAZ_00047005"/>
        <obo:RO_0001025 rdf:resource="http://purl.obolibrary.org/obo/GAZ_00147196"/>
        <obo:IAO_0000115>The easternmost of three large bays lying on the Foveaux Strait coast of Southland, New Zealand. Thirty km in length, the bay is the southern end of the Awarua Plain, an area of swampy land stretching inland for about fifteen km. The eastern end of the bay is close to Slope Point, the South Island&apos;s southernmost point, and the start of the Catlins.</obo:IAO_0000115>
        <oboInOwl:hasOBONamespace>GAZ</oboInOwl:hasOBONamespace>
        <oboInOwl:id>GAZ:00142664</oboInOwl:id>
        <rdfs:label>Toetoes Bay</rdfs:label>
    </owl:NamedIndividual>
    


    <!-- http://purl.obolibrary.org/obo/GAZ_00142665 -->

    <owl:NamedIndividual rdf:about="http://purl.obolibrary.org/obo/GAZ_00142665">
        <obo:RO_0001025 rdf:resource="http://purl.obolibrary.org/obo/GAZ_00047005"/>
        <obo:IAO_0000115>The westernmost of three large bays lying on the Foveaux Strait coast of Southland, New Zealand. Twenty-seven km in length, the western end of the bay is mountainous, with the southern terminus of the Southern Alps and Fiordland National Park.</obo:IAO_0000115>
        <oboInOwl:hasOBONamespace>GAZ</oboInOwl:hasOBONamespace>
        <oboInOwl:id>GAZ:00142665</oboInOwl:id>
        <rdfs:label>Te Waewae Bay</rdfs:label>
    </owl:NamedIndividual>
    


    <!-- http://purl.obolibrary.org/obo/GAZ_00142666 -->

    <owl:NamedIndividual rdf:about="http://purl.obolibrary.org/obo/GAZ_00142666">
        <obo:RO_0001025 rdf:resource="http://purl.obolibrary.org/obo/GAZ_00047005"/>
        <obo:IAO_0000115>The central bay of three lying on the Foveaux Strait coast of Southland, New Zealand, the others being Te Waewae Bay and Toetoes Bay. Twenty-six km in length, the bay lies between the town of Riverton and the outflow of the Aparima River in the northwest, and the estuary of the Oreti River in the southeast.</obo:IAO_0000115>
        <oboInOwl:hasOBONamespace>GAZ</oboInOwl:hasOBONamespace>
        <oboInOwl:id>GAZ:00142666</oboInOwl:id>
        <rdfs:label>Oreti Beach</rdfs:label>
    </owl:NamedIndividual>
    


    <!-- http://purl.obolibrary.org/obo/GAZ_00142667 -->

    <owl:NamedIndividual rdf:about="http://purl.obolibrary.org/obo/GAZ_00142667">
        <obo:RO_0001025 rdf:resource="http://purl.obolibrary.org/obo/GAZ_00142664"/>
        <obo:IAO_0000115>A lagoon opening into Toetoes Bay.</obo:IAO_0000115>
        <oboInOwl:hasOBONamespace>GAZ</oboInOwl:hasOBONamespace>
        <oboInOwl:id>GAZ:00142667</oboInOwl:id>
        <rdfs:label>Waituna Lagoon</rdfs:label>
    </owl:NamedIndividual>
    


    <!-- http://purl.obolibrary.org/obo/GAZ_00142668 -->

    <owl:NamedIndividual rdf:about="http://purl.obolibrary.org/obo/GAZ_00142668">
        <obo:RO_0001025 rdf:resource="http://purl.obolibrary.org/obo/GAZ_00047005"/>
        <obo:IAO_0000115>A small island S of Bluff Harbour.</obo:IAO_0000115>
        <oboInOwl:hasOBONamespace>GAZ</oboInOwl:hasOBONamespace>
        <oboInOwl:id>GAZ:00142668</oboInOwl:id>
        <rdfs:label>Dog Island</rdfs:label>
    </owl:NamedIndividual>
    


    <!-- http://purl.obolibrary.org/obo/GAZ_00142669 -->

    <owl:NamedIndividual rdf:about="http://purl.obolibrary.org/obo/GAZ_00142669">
        <obo:RO_0001025 rdf:resource="http://purl.obolibrary.org/obo/GAZ_00047005"/>
        <obo:IAO_0000115>An estuary opening into Foveaux Strait at Invercargill.</obo:IAO_0000115>
        <oboInOwl:hasOBONamespace>GAZ</oboInOwl:hasOBONamespace>
        <oboInOwl:id>GAZ:00142669</oboInOwl:id>
        <rdfs:label>New River Estuary</rdfs:label>
    </owl:NamedIndividual>
    


    <!-- http://purl.obolibrary.org/obo/GAZ_00142670 -->

    <owl:NamedIndividual rdf:about="http://purl.obolibrary.org/obo/GAZ_00142670">
        <obo:RO_0001025 rdf:resource="http://purl.obolibrary.org/obo/GAZ_00047005"/>
        <obo:IAO_0000115>A bay S of Invercargill.</obo:IAO_0000115>
        <oboInOwl:hasOBONamespace>GAZ</oboInOwl:hasOBONamespace>
        <oboInOwl:id>GAZ:00142670</oboInOwl:id>
        <rdfs:label>Bluff Harbour</rdfs:label>
    </owl:NamedIndividual>
    


    <!-- http://purl.obolibrary.org/obo/GAZ_00142671 -->

    <owl:NamedIndividual rdf:about="http://purl.obolibrary.org/obo/GAZ_00142671">
        <obo:RO_0001025 rdf:resource="http://purl.obolibrary.org/obo/GAZ_00047005"/>
        <obo:IAO_0000115>A small island SW of Riverton.</obo:IAO_0000115>
        <oboInOwl:hasOBONamespace>GAZ</oboInOwl:hasOBONamespace>
        <oboInOwl:id>GAZ:00142671</oboInOwl:id>
        <rdfs:label>Pig Island</rdfs:label>
    </owl:NamedIndividual>
    


    <!-- http://purl.obolibrary.org/obo/GAZ_00142672 -->

    <owl:NamedIndividual rdf:about="http://purl.obolibrary.org/obo/GAZ_00142672">
        <obo:RO_0001025 rdf:resource="http://purl.obolibrary.org/obo/GAZ_00047005"/>
        <obo:IAO_0000115>Reefs S of Pig Island.</obo:IAO_0000115>
        <oboInOwl:hasOBONamespace>GAZ</oboInOwl:hasOBONamespace>
        <oboInOwl:id>GAZ:00142672</oboInOwl:id>
        <rdfs:label>Esacpe Reefs</rdfs:label>
    </owl:NamedIndividual>
    


    <!-- http://purl.obolibrary.org/obo/GAZ_00142673 -->

    <owl:NamedIndividual rdf:about="http://purl.obolibrary.org/obo/GAZ_00142673">
        <obo:RO_0001025 rdf:resource="http://purl.obolibrary.org/obo/GAZ_00047005"/>
        <obo:IAO_0000115>An island S of Colac.</obo:IAO_0000115>
        <oboInOwl:hasOBONamespace>GAZ</oboInOwl:hasOBONamespace>
        <oboInOwl:id>GAZ:00142673</oboInOwl:id>
        <rdfs:label>Centre Island</rdfs:label>
    </owl:NamedIndividual>
    


    <!-- http://purl.obolibrary.org/obo/GAZ_00142678 -->

    <owl:NamedIndividual rdf:about="http://purl.obolibrary.org/obo/GAZ_00142678">
        <obo:RO_0001025 rdf:resource="http://purl.obolibrary.org/obo/GAZ_00046921"/>
        <obo:IAO_0000115>A long narrow peninsula on the west coast of Resolution Island.</obo:IAO_0000115>
        <oboInOwl:hasOBONamespace>GAZ</oboInOwl:hasOBONamespace>
        <oboInOwl:id>GAZ:00142678</oboInOwl:id>
        <rdfs:label>Five Fingers Peninsula</rdfs:label>
    </owl:NamedIndividual>
    


    <!-- http://purl.obolibrary.org/obo/GAZ_00142703 -->

    <owl:NamedIndividual rdf:about="http://purl.obolibrary.org/obo/GAZ_00142703">
        <obo:RO_0001025 rdf:resource="http://purl.obolibrary.org/obo/GAZ_00004777"/>
        <obo:IAO_0000115>A coastal lagoon on the West Coast of New Zealand&apos;s South Island. It is located 130 km south of Hokitika. Several small rivers drain into the lagoon, and it is the outflow of Lake Mapourika.</obo:IAO_0000115>
        <oboInOwl:hasOBONamespace>GAZ</oboInOwl:hasOBONamespace>
        <oboInOwl:id>GAZ:00142703</oboInOwl:id>
        <rdfs:label>Okarito Lagoon</rdfs:label>
    </owl:NamedIndividual>
    


    <!-- http://purl.obolibrary.org/obo/GAZ_00142708 -->

    <owl:NamedIndividual rdf:about="http://purl.obolibrary.org/obo/GAZ_00142708">
        <obo:RO_0001025 rdf:resource="http://purl.obolibrary.org/obo/GAZ_00047000"/>
        <obo:IAO_0000115>A bay in the NW of Tasman Bay, S of Separation Point.</obo:IAO_0000115>
        <oboInOwl:hasOBONamespace>GAZ</oboInOwl:hasOBONamespace>
        <oboInOwl:id>GAZ:00142708</oboInOwl:id>
        <rdfs:label>Awaroa Bay</rdfs:label>
    </owl:NamedIndividual>
    


    <!-- http://purl.obolibrary.org/obo/GAZ_00142709 -->

    <owl:NamedIndividual rdf:about="http://purl.obolibrary.org/obo/GAZ_00142709">
        <obo:RO_0001025 rdf:resource="http://purl.obolibrary.org/obo/GAZ_00047000"/>
        <obo:IAO_0000115>A bay in the NE of Tasman Bay.</obo:IAO_0000115>
        <oboInOwl:hasOBONamespace>GAZ</oboInOwl:hasOBONamespace>
        <oboInOwl:id>GAZ:00142709</oboInOwl:id>
        <rdfs:label>Delaware Bay</rdfs:label>
    </owl:NamedIndividual>
    


    <!-- http://purl.obolibrary.org/obo/GAZ_00142710 -->

    <owl:NamedIndividual rdf:about="http://purl.obolibrary.org/obo/GAZ_00142710">
        <obo:RO_0001025 rdf:resource="http://purl.obolibrary.org/obo/GAZ_00047000"/>
        <obo:IAO_0000115>A small island in the W of Tasman Bay.</obo:IAO_0000115>
        <oboInOwl:hasOBONamespace>GAZ</oboInOwl:hasOBONamespace>
        <oboInOwl:id>GAZ:00142710</oboInOwl:id>
        <rdfs:label>Adele Island</rdfs:label>
    </owl:NamedIndividual>
    


    <!-- http://purl.obolibrary.org/obo/GAZ_00142711 -->

    <owl:NamedIndividual rdf:about="http://purl.obolibrary.org/obo/GAZ_00142711">
        <obo:RO_0001025 rdf:resource="http://purl.obolibrary.org/obo/GAZ_00047000"/>
        <obo:IAO_0000115>A small island in the NW of Tasman Bay.</obo:IAO_0000115>
        <oboInOwl:hasOBONamespace>GAZ</oboInOwl:hasOBONamespace>
        <oboInOwl:id>GAZ:00142711</oboInOwl:id>
        <rdfs:label>Tonga Island</rdfs:label>
    </owl:NamedIndividual>
    


    <!-- http://purl.obolibrary.org/obo/GAZ_00142712 -->

    <owl:NamedIndividual rdf:about="http://purl.obolibrary.org/obo/GAZ_00142712">
        <obo:RO_0001025 rdf:resource="http://purl.obolibrary.org/obo/GAZ_00142709"/>
        <obo:IAO_0000115>An island in the SW of Delaware Bay.</obo:IAO_0000115>
        <oboInOwl:hasOBONamespace>GAZ</oboInOwl:hasOBONamespace>
        <oboInOwl:id>GAZ:00142712</oboInOwl:id>
        <rdfs:label>Pepin Island</rdfs:label>
    </owl:NamedIndividual>
    


    <!-- http://purl.obolibrary.org/obo/GAZ_00142713 -->

    <owl:NamedIndividual rdf:about="http://purl.obolibrary.org/obo/GAZ_00142713">
        <obo:RO_0001025 rdf:resource="http://purl.obolibrary.org/obo/GAZ_00046925"/>
        <obo:IAO_0000115>A bay E of Cape Soucis.</obo:IAO_0000115>
        <oboInOwl:hasOBONamespace>GAZ</oboInOwl:hasOBONamespace>
        <oboInOwl:id>GAZ:00142713</oboInOwl:id>
        <rdfs:label>Croiselles Harbour</rdfs:label>
    </owl:NamedIndividual>
    


    <!-- http://purl.obolibrary.org/obo/GAZ_00142714 -->

    <owl:NamedIndividual rdf:about="http://purl.obolibrary.org/obo/GAZ_00142714">
        <obo:RO_0001025 rdf:resource="http://purl.obolibrary.org/obo/GAZ_00046925"/>
        <obo:IAO_0000115>The easternmost of the main sounds of the Marlborough Sounds, in New Zealand&apos;s South Island. It is, like the other sounds, a drowned valley, and like the majority of its neighbours it runs southwest to northeast before joining Cook Strait.</obo:IAO_0000115>
        <oboInOwl:hasOBONamespace>GAZ</oboInOwl:hasOBONamespace>
        <oboInOwl:id>GAZ:00142714</oboInOwl:id>
        <rdfs:label>Queen Charlotte Sound</rdfs:label>
    </owl:NamedIndividual>
    


    <!-- http://purl.obolibrary.org/obo/GAZ_00142715 -->

    <owl:NamedIndividual rdf:about="http://purl.obolibrary.org/obo/GAZ_00142715">
        <obo:RO_0001025 rdf:resource="http://purl.obolibrary.org/obo/GAZ_00046925"/>
        <obo:IAO_0000115>One of the drowned valleys that form the Marlborough Sounds in New Zealand.</obo:IAO_0000115>
        <oboInOwl:hasOBONamespace>GAZ</oboInOwl:hasOBONamespace>
        <oboInOwl:id>GAZ:00142715</oboInOwl:id>
        <rdfs:label>Tory Channel</rdfs:label>
    </owl:NamedIndividual>
    


    <!-- http://purl.obolibrary.org/obo/GAZ_00142716 -->

    <owl:NamedIndividual rdf:about="http://purl.obolibrary.org/obo/GAZ_00142716">
        <obo:RO_0001025 rdf:resource="http://purl.obolibrary.org/obo/GAZ_00142717"/>
        <obo:IAO_0000115>One of the larger of the Marlborough Sounds in the South Island of New Zealand. The drowned valley is an arm of Pelorus Sound, it runs for 25 km from the northeast to southwest, joining Pelorus Sound a quarter of the way down the latter&apos;s path to the Cook Strait.</obo:IAO_0000115>
        <oboInOwl:hasOBONamespace>GAZ</oboInOwl:hasOBONamespace>
        <oboInOwl:id>GAZ:00142716</oboInOwl:id>
        <rdfs:label>Kenepuru Sound</rdfs:label>
    </owl:NamedIndividual>
    


    <!-- http://purl.obolibrary.org/obo/GAZ_00142717 -->

    <owl:NamedIndividual rdf:about="http://purl.obolibrary.org/obo/GAZ_00142717">
        <obo:RO_0001025 rdf:resource="http://purl.obolibrary.org/obo/GAZ_00046925"/>
        <obo:IAO_0000115>A long-drowned valley in the Marlborough Sounds in New Zealand.</obo:IAO_0000115>
        <oboInOwl:hasOBONamespace>GAZ</oboInOwl:hasOBONamespace>
        <oboInOwl:id>GAZ:00142717</oboInOwl:id>
        <rdfs:label>Pelorus Sound</rdfs:label>
    </owl:NamedIndividual>
    


    <!-- http://purl.obolibrary.org/obo/GAZ_00142718 -->

    <owl:NamedIndividual rdf:about="http://purl.obolibrary.org/obo/GAZ_00142718">
        <obo:RO_0001025 rdf:resource="http://purl.obolibrary.org/obo/GAZ_00142717"/>
        <obo:IAO_0000115>THe southern arm of Pelorus Sound in the Marlborough Sounds. Tennyson Inlet encompasses Duncan Bay to Tawhitinui Reach.</obo:IAO_0000115>
        <oboInOwl:hasOBONamespace>GAZ</oboInOwl:hasOBONamespace>
        <oboInOwl:id>GAZ:00142718</oboInOwl:id>
        <rdfs:label>Tennyson Inlet</rdfs:label>
    </owl:NamedIndividual>
    


    <!-- http://purl.obolibrary.org/obo/GAZ_00142719 -->

    <owl:NamedIndividual rdf:about="http://purl.obolibrary.org/obo/GAZ_00142719">
        <obo:RO_0001025 rdf:resource="http://purl.obolibrary.org/obo/GAZ_00142718"/>
        <obo:IAO_0000115>An island in Tennyson Inlet.</obo:IAO_0000115>
        <oboInOwl:hasOBONamespace>GAZ</oboInOwl:hasOBONamespace>
        <oboInOwl:id>GAZ:00142719</oboInOwl:id>
        <rdfs:label>Tarakaipa Island</rdfs:label>
    </owl:NamedIndividual>
    


    <!-- http://purl.obolibrary.org/obo/GAZ_00142720 -->

    <owl:NamedIndividual rdf:about="http://purl.obolibrary.org/obo/GAZ_00142720">
        <obo:RO_0001025 rdf:resource="http://purl.obolibrary.org/obo/GAZ_00142718"/>
        <obo:IAO_0000115>An island in Tennyson Inlet.</obo:IAO_0000115>
        <oboInOwl:hasOBONamespace>GAZ</oboInOwl:hasOBONamespace>
        <oboInOwl:id>GAZ:00142720</oboInOwl:id>
        <rdfs:label>Tawhitinui Island</rdfs:label>
    </owl:NamedIndividual>
    


    <!-- http://purl.obolibrary.org/obo/GAZ_00142721 -->

    <owl:NamedIndividual rdf:about="http://purl.obolibrary.org/obo/GAZ_00142721">
        <rdf:type rdf:resource="http://purl.obolibrary.org/obo/ENVO_00000475"/>
        <obo:RO_0001025 rdf:resource="http://purl.obolibrary.org/obo/GAZ_00142717"/>
        <obo:IAO_0000115>An arm of Pelorus Sound.</obo:IAO_0000115>
        <oboInOwl:hasOBONamespace>GAZ</oboInOwl:hasOBONamespace>
        <oboInOwl:id>GAZ:00142721</oboInOwl:id>
        <rdfs:label>Tawhitinui Reach</rdfs:label>
    </owl:NamedIndividual>
    


    <!-- http://purl.obolibrary.org/obo/GAZ_00142722 -->

    <owl:NamedIndividual rdf:about="http://purl.obolibrary.org/obo/GAZ_00142722">
        <obo:RO_0001025 rdf:resource="http://purl.obolibrary.org/obo/GAZ_00046925"/>
        <obo:IAO_0000115>The strait between the mainland of South Island and D&apos;Urville Island.</obo:IAO_0000115>
        <oboInOwl:hasOBONamespace>GAZ</oboInOwl:hasOBONamespace>
        <oboInOwl:id>GAZ:00142722</oboInOwl:id>
        <rdfs:label>French Pass</rdfs:label>
    </owl:NamedIndividual>
    


    <!-- http://purl.obolibrary.org/obo/GAZ_00142723 -->

    <owl:NamedIndividual rdf:about="http://purl.obolibrary.org/obo/GAZ_00142723">
        <obo:RO_0001025 rdf:resource="http://purl.obolibrary.org/obo/GAZ_00016679"/>
        <obo:IAO_0000115>The W point of D&apos;Urville Island.</obo:IAO_0000115>
        <oboInOwl:hasOBONamespace>GAZ</oboInOwl:hasOBONamespace>
        <oboInOwl:id>GAZ:00142723</oboInOwl:id>
        <rdfs:label>Ragged Point</rdfs:label>
    </owl:NamedIndividual>
    


    <!-- http://purl.obolibrary.org/obo/GAZ_00142724 -->

    <owl:NamedIndividual rdf:about="http://purl.obolibrary.org/obo/GAZ_00142724">
        <obo:RO_0001025 rdf:resource="http://purl.obolibrary.org/obo/GAZ_00016679"/>
        <obo:IAO_0000115>The N point of D&apos;Urville Island.</obo:IAO_0000115>
        <oboInOwl:hasOBONamespace>GAZ</oboInOwl:hasOBONamespace>
        <oboInOwl:id>GAZ:00142724</oboInOwl:id>
        <rdfs:label>Cape Stephens</rdfs:label>
    </owl:NamedIndividual>
    


    <!-- http://purl.obolibrary.org/obo/GAZ_00142725 -->

    <owl:NamedIndividual rdf:about="http://purl.obolibrary.org/obo/GAZ_00142725">
        <obo:RO_0001025 rdf:resource="http://purl.obolibrary.org/obo/GAZ_00046925"/>
        <obo:IAO_0000115>Islands N of Forsyth Island.</obo:IAO_0000115>
        <oboInOwl:hasOBONamespace>GAZ</oboInOwl:hasOBONamespace>
        <oboInOwl:id>GAZ:00142725</oboInOwl:id>
        <rdfs:label>Chetwood Islands</rdfs:label>
    </owl:NamedIndividual>
    


    <!-- http://purl.obolibrary.org/obo/GAZ_00142726 -->

    <owl:NamedIndividual rdf:about="http://purl.obolibrary.org/obo/GAZ_00142726">
        <obo:RO_0001025 rdf:resource="http://purl.obolibrary.org/obo/GAZ_00046925"/>
        <obo:IAO_0000115>A bay on the N coast of South Island, N of Mount Shewell.</obo:IAO_0000115>
        <oboInOwl:hasOBONamespace>GAZ</oboInOwl:hasOBONamespace>
        <oboInOwl:id>GAZ:00142726</oboInOwl:id>
        <rdfs:label>Admiralty Bay</rdfs:label>
    </owl:NamedIndividual>
    


    <!-- http://purl.obolibrary.org/obo/GAZ_00142727 -->

    <owl:NamedIndividual rdf:about="http://purl.obolibrary.org/obo/GAZ_00142727">
        <obo:RO_0001025 rdf:resource="http://purl.obolibrary.org/obo/GAZ_00046925"/>
        <obo:IAO_0000115>An island W of Alligator Head.</obo:IAO_0000115>
        <oboInOwl:hasOBONamespace>GAZ</oboInOwl:hasOBONamespace>
        <oboInOwl:id>GAZ:00142727</oboInOwl:id>
        <rdfs:label>Forsyth Island</rdfs:label>
    </owl:NamedIndividual>
    


    <!-- http://purl.obolibrary.org/obo/GAZ_00142728 -->

    <owl:NamedIndividual rdf:about="http://purl.obolibrary.org/obo/GAZ_00142728">
        <obo:RO_0001025 rdf:resource="http://purl.obolibrary.org/obo/GAZ_00046925"/>
        <obo:IAO_0000115>An island off the NE coast of D&apos;Urville Island.</obo:IAO_0000115>
        <oboInOwl:hasOBONamespace>GAZ</oboInOwl:hasOBONamespace>
        <oboInOwl:id>GAZ:00142728</oboInOwl:id>
        <rdfs:label>Rangitoo Island</rdfs:label>
    </owl:NamedIndividual>
    


    <!-- http://purl.obolibrary.org/obo/GAZ_00142729 -->

    <owl:NamedIndividual rdf:about="http://purl.obolibrary.org/obo/GAZ_00142729">
        <obo:RO_0001025 rdf:resource="http://purl.obolibrary.org/obo/GAZ_00046925"/>
        <obo:IAO_0000115>A bay between Alligator Head and Cape Jackson.</obo:IAO_0000115>
        <oboInOwl:hasOBONamespace>GAZ</oboInOwl:hasOBONamespace>
        <oboInOwl:id>GAZ:00142729</oboInOwl:id>
        <rdfs:label>Port Gore</rdfs:label>
    </owl:NamedIndividual>
    


    <!-- http://purl.obolibrary.org/obo/GAZ_00142730 -->

    <owl:NamedIndividual rdf:about="http://purl.obolibrary.org/obo/GAZ_00142730">
        <obo:RO_0001025 rdf:resource="http://purl.obolibrary.org/obo/GAZ_00142714"/>
        <obo:IAO_0000115>A small island in the mouth of Queen Charlotte Sound.</obo:IAO_0000115>
        <oboInOwl:hasOBONamespace>GAZ</oboInOwl:hasOBONamespace>
        <oboInOwl:id>GAZ:00142730</oboInOwl:id>
        <rdfs:label>Blumine Island</rdfs:label>
    </owl:NamedIndividual>
    


    <!-- http://purl.obolibrary.org/obo/GAZ_00142731 -->

    <owl:NamedIndividual rdf:about="http://purl.obolibrary.org/obo/GAZ_00142731">
        <obo:RO_0001025 rdf:resource="http://purl.obolibrary.org/obo/GAZ_00046929"/>
        <obo:IAO_0000115>A bay, facing Cook Strait, located at the northeast of New Zealand&apos;s South Island, to the south of the Marlborough Sounds.</obo:IAO_0000115>
        <oboInOwl:hasOBONamespace>GAZ</oboInOwl:hasOBONamespace>
        <oboInOwl:id>GAZ:00142731</oboInOwl:id>
        <rdfs:label>Cloudy Bay</rdfs:label>
    </owl:NamedIndividual>
    


    <!-- http://purl.obolibrary.org/obo/GAZ_00142732 -->

    <owl:NamedIndividual rdf:about="http://purl.obolibrary.org/obo/GAZ_00142732">
        <obo:RO_0001025 rdf:resource="http://purl.obolibrary.org/obo/GAZ_00046929"/>
        <obo:IAO_0000115>A bay in the northeast of the South Island of New Zealand, in the Marlborough region. It lies between Cloudy Bay to the northwest, and Cape Campbell, the easternmost point of the South Island.</obo:IAO_0000115>
        <oboInOwl:hasOBONamespace>GAZ</oboInOwl:hasOBONamespace>
        <oboInOwl:id>GAZ:00142732</oboInOwl:id>
        <rdfs:label>Clifford Bay</rdfs:label>
    </owl:NamedIndividual>
    


    <!-- http://purl.obolibrary.org/obo/GAZ_00142739 -->

    <owl:NamedIndividual rdf:about="http://purl.obolibrary.org/obo/GAZ_00142739">
        <obo:RO_0001025 rdf:resource="http://purl.obolibrary.org/obo/GAZ_00008565"/>
        <obo:RO_0001025 rdf:resource="http://purl.obolibrary.org/obo/GAZ_00046929"/>
        <obo:IAO_0000115>A suburb on the south side of the Rongotai isthmus in Wellington, New Zealand.</obo:IAO_0000115>
        <oboInOwl:hasOBONamespace>GAZ</oboInOwl:hasOBONamespace>
        <oboInOwl:id>GAZ:00142739</oboInOwl:id>
        <rdfs:label>Lyall Bay</rdfs:label>
    </owl:NamedIndividual>
    


    <!-- http://purl.obolibrary.org/obo/GAZ_00142744 -->

    <owl:NamedIndividual rdf:about="http://purl.obolibrary.org/obo/GAZ_00142744">
        <obo:RO_0001025 rdf:resource="http://purl.obolibrary.org/obo/GAZ_00030235"/>
        <obo:IAO_0000115>Rocks to the N of Whakaari Island in the Bay of Plenty.</obo:IAO_0000115>
        <oboInOwl:hasOBONamespace>GAZ</oboInOwl:hasOBONamespace>
        <oboInOwl:id>GAZ:00142744</oboInOwl:id>
        <rdfs:label>Volkner Rocks</rdfs:label>
    </owl:NamedIndividual>
    


    <!-- http://purl.obolibrary.org/obo/GAZ_00142745 -->

    <owl:NamedIndividual rdf:about="http://purl.obolibrary.org/obo/GAZ_00142745">
        <obo:RO_0001025 rdf:resource="http://purl.obolibrary.org/obo/GAZ_00030230"/>
        <obo:IAO_0000115>A bay in the E of the Bay of Plenty.</obo:IAO_0000115>
        <oboInOwl:hasOBONamespace>GAZ</oboInOwl:hasOBONamespace>
        <oboInOwl:id>GAZ:00142745</oboInOwl:id>
        <rdfs:label>Omaio Bay</rdfs:label>
    </owl:NamedIndividual>
    


    <!-- http://purl.obolibrary.org/obo/GAZ_00142746 -->

    <owl:NamedIndividual rdf:about="http://purl.obolibrary.org/obo/GAZ_00142746">
        <obo:RO_0001025 rdf:resource="http://purl.obolibrary.org/obo/GAZ_00030230"/>
        <obo:IAO_0000115>A large harbour separated from the Bay of Plenty by Matakana Island.</obo:IAO_0000115>
        <oboInOwl:hasOBONamespace>GAZ</oboInOwl:hasOBONamespace>
        <oboInOwl:id>GAZ:00142746</oboInOwl:id>
        <rdfs:label>Tauranga Harbour</rdfs:label>
    </owl:NamedIndividual>
    


    <!-- http://purl.obolibrary.org/obo/GAZ_00142747 -->

    <owl:NamedIndividual rdf:about="http://purl.obolibrary.org/obo/GAZ_00142747">
        <obo:RO_0001025 rdf:resource="http://purl.obolibrary.org/obo/GAZ_00030230"/>
        <obo:IAO_0000115>A bay in the E of the Bay of Plenty.</obo:IAO_0000115>
        <oboInOwl:hasOBONamespace>GAZ</oboInOwl:hasOBONamespace>
        <oboInOwl:id>GAZ:00142747</oboInOwl:id>
        <rdfs:label>Papatea Bay</rdfs:label>
    </owl:NamedIndividual>
    


    <!-- http://purl.obolibrary.org/obo/GAZ_00142748 -->

    <owl:NamedIndividual rdf:about="http://purl.obolibrary.org/obo/GAZ_00142748">
        <obo:RO_0001025 rdf:resource="http://purl.obolibrary.org/obo/GAZ_00030230"/>
        <oboInOwl:hasOBONamespace>GAZ</oboInOwl:hasOBONamespace>
        <oboInOwl:id>GAZ:00142748</oboInOwl:id>
        <rdfs:label>Whangaparaoa Bay</rdfs:label>
    </owl:NamedIndividual>
    


    <!-- http://purl.obolibrary.org/obo/GAZ_00142749 -->

    <owl:NamedIndividual rdf:about="http://purl.obolibrary.org/obo/GAZ_00142749">
        <obo:RO_0001025 rdf:resource="http://purl.obolibrary.org/obo/GAZ_00030230"/>
        <obo:IAO_0000115>An inlet in the S of the Bay of Plenty, E of the town of Whakane.</obo:IAO_0000115>
        <oboInOwl:hasOBONamespace>GAZ</oboInOwl:hasOBONamespace>
        <oboInOwl:id>GAZ:00142749</oboInOwl:id>
        <rdfs:label>Ohiwa Harbour</rdfs:label>
    </owl:NamedIndividual>
    


    <!-- http://purl.obolibrary.org/obo/GAZ_00142750 -->

    <owl:NamedIndividual rdf:about="http://purl.obolibrary.org/obo/GAZ_00142750">
        <obo:RO_0001025 rdf:resource="http://purl.obolibrary.org/obo/GAZ_00030235"/>
        <obo:IAO_0000115>A small island N of the town of Whakatane.</obo:IAO_0000115>
        <oboInOwl:hasOBONamespace>GAZ</oboInOwl:hasOBONamespace>
        <oboInOwl:id>GAZ:00142750</oboInOwl:id>
        <rdfs:label>Motuhora Island</rdfs:label>
    </owl:NamedIndividual>
    


    <!-- http://purl.obolibrary.org/obo/GAZ_00142751 -->

    <owl:NamedIndividual rdf:about="http://purl.obolibrary.org/obo/GAZ_00142751">
        <obo:RO_0001025 rdf:resource="http://purl.obolibrary.org/obo/GAZ_00030230"/>
        <obo:IAO_0000115>An inlet in the NW of the Bay of Plenty, on the E side of the Coromandel Peninsula.</obo:IAO_0000115>
        <oboInOwl:hasOBONamespace>GAZ</oboInOwl:hasOBONamespace>
        <oboInOwl:id>GAZ:00142751</oboInOwl:id>
        <rdfs:label>Tairua Harbour</rdfs:label>
    </owl:NamedIndividual>
    


    <!-- http://purl.obolibrary.org/obo/GAZ_00142752 -->

    <owl:NamedIndividual rdf:about="http://purl.obolibrary.org/obo/GAZ_00142752">
        <obo:RO_0001025 rdf:resource="http://purl.obolibrary.org/obo/GAZ_00030235"/>
        <obo:IAO_0000115>An island located three km to the east of the Coromandel Peninsula in New Zealand&apos;s North Island and eight km southeast of the town of Pauanui.</obo:IAO_0000115>
        <oboInOwl:hasOBONamespace>GAZ</oboInOwl:hasOBONamespace>
        <oboInOwl:id>GAZ:00142752</oboInOwl:id>
        <rdfs:label>Slipper Island</rdfs:label>
    </owl:NamedIndividual>
    


    <!-- http://purl.obolibrary.org/obo/GAZ_00142753 -->

    <owl:NamedIndividual rdf:about="http://purl.obolibrary.org/obo/GAZ_00142753">
        <obo:RO_0001025 rdf:resource="http://purl.obolibrary.org/obo/GAZ_00030235"/>
        <obo:IAO_0000115>A small island NW of Motuhora Island.</obo:IAO_0000115>
        <oboInOwl:hasOBONamespace>GAZ</oboInOwl:hasOBONamespace>
        <oboInOwl:id>GAZ:00142753</oboInOwl:id>
        <rdfs:label>Moutoki Island</rdfs:label>
    </owl:NamedIndividual>
    


    <!-- http://purl.obolibrary.org/obo/GAZ_00142754 -->

    <owl:NamedIndividual rdf:about="http://purl.obolibrary.org/obo/GAZ_00142754">
        <obo:RO_0001025 rdf:resource="http://purl.obolibrary.org/obo/GAZ_00030235"/>
        <obo:IAO_0000115>An island in the NW of the Bay of Plenty.</obo:IAO_0000115>
        <oboInOwl:hasOBONamespace>GAZ</oboInOwl:hasOBONamespace>
        <oboInOwl:id>GAZ:00142754</oboInOwl:id>
        <rdfs:label>Ohinau Island</rdfs:label>
    </owl:NamedIndividual>
    


    <!-- http://purl.obolibrary.org/obo/GAZ_00142755 -->

    <owl:NamedIndividual rdf:about="http://purl.obolibrary.org/obo/GAZ_00142755">
        <obo:RO_0001025 rdf:resource="http://purl.obolibrary.org/obo/GAZ_00030235"/>
        <obo:IAO_0000115>A small island SE of Motiti Island.</obo:IAO_0000115>
        <oboInOwl:hasOBONamespace>GAZ</oboInOwl:hasOBONamespace>
        <oboInOwl:id>GAZ:00142755</oboInOwl:id>
        <rdfs:label>Plate Island</rdfs:label>
    </owl:NamedIndividual>
    


    <!-- http://purl.obolibrary.org/obo/GAZ_00142756 -->

    <owl:NamedIndividual rdf:about="http://purl.obolibrary.org/obo/GAZ_00142756">
        <obo:RO_0001025 rdf:resource="http://purl.obolibrary.org/obo/GAZ_00030235"/>
        <obo:IAO_0000115>A small island off Matakana Island.</obo:IAO_0000115>
        <oboInOwl:hasOBONamespace>GAZ</oboInOwl:hasOBONamespace>
        <oboInOwl:id>GAZ:00142756</oboInOwl:id>
        <rdfs:label>Karewa Island</rdfs:label>
    </owl:NamedIndividual>
    


    <!-- http://purl.obolibrary.org/obo/GAZ_00142757 -->

    <owl:NamedIndividual rdf:about="http://purl.obolibrary.org/obo/GAZ_00142757">
        <obo:RO_0001025 rdf:resource="http://purl.obolibrary.org/obo/GAZ_00142746"/>
        <obo:IAO_0000115>An entrance to Tauranga Harbor, N of Matakana Island.</obo:IAO_0000115>
        <oboInOwl:hasOBONamespace>GAZ</oboInOwl:hasOBONamespace>
        <oboInOwl:id>GAZ:00142757</oboInOwl:id>
        <rdfs:label>Katikati Entrance</rdfs:label>
    </owl:NamedIndividual>
    


    <!-- http://purl.obolibrary.org/obo/GAZ_00142758 -->

    <owl:NamedIndividual rdf:about="http://purl.obolibrary.org/obo/GAZ_00142758">
        <obo:RO_0001025 rdf:resource="http://purl.obolibrary.org/obo/GAZ_00030235"/>
        <obo:IAO_0000115>A small island in the NW of the Bay of Plenty, off Tairua Harbour.</obo:IAO_0000115>
        <oboInOwl:hasOBONamespace>GAZ</oboInOwl:hasOBONamespace>
        <oboInOwl:id>GAZ:00142758</oboInOwl:id>
        <rdfs:label>Shoe Island</rdfs:label>
    </owl:NamedIndividual>
    


    <!-- http://purl.obolibrary.org/obo/GAZ_00142759 -->

    <owl:NamedIndividual rdf:about="http://purl.obolibrary.org/obo/GAZ_00142759">
        <obo:RO_0001025 rdf:resource="http://purl.obolibrary.org/obo/GAZ_00046945"/>
        <obo:IAO_0000115>One of three channels connecting the Hauraki Gulf with the Pacific Ocean to the northeast of Auckland, New Zealand. It is the central channel, lying between Great Barrier Island to the east and Hauturu/Little Barrier Island to the west.</obo:IAO_0000115>
        <oboInOwl:hasOBONamespace>GAZ</oboInOwl:hasOBONamespace>
        <oboInOwl:id>GAZ:00142759</oboInOwl:id>
        <rdfs:label>Cradock Channel</rdfs:label>
    </owl:NamedIndividual>
    


    <!-- http://purl.obolibrary.org/obo/GAZ_00142761 -->

    <owl:NamedIndividual rdf:about="http://purl.obolibrary.org/obo/GAZ_00142761">
        <obo:RO_0001025 rdf:resource="http://purl.obolibrary.org/obo/GAZ_00046945"/>
        <obo:IAO_0000115>A bay on the NW of Great Barrier Island.</obo:IAO_0000115>
        <oboInOwl:hasOBONamespace>GAZ</oboInOwl:hasOBONamespace>
        <oboInOwl:id>GAZ:00142761</oboInOwl:id>
        <rdfs:label>Katherine Bay</rdfs:label>
    </owl:NamedIndividual>
    


    <!-- http://purl.obolibrary.org/obo/GAZ_00142763 -->

    <owl:NamedIndividual rdf:about="http://purl.obolibrary.org/obo/GAZ_00142763">
        <obo:RO_0001025 rdf:resource="http://purl.obolibrary.org/obo/GAZ_00046945"/>
        <obo:IAO_0000115>A bay in the SW of Great Barrier Island.</obo:IAO_0000115>
        <oboInOwl:hasOBONamespace>GAZ</oboInOwl:hasOBONamespace>
        <oboInOwl:id>GAZ:00142763</oboInOwl:id>
        <rdfs:label>Tryphena Harbour</rdfs:label>
    </owl:NamedIndividual>
    


    <!-- http://purl.obolibrary.org/obo/GAZ_00142764 -->

    <owl:NamedIndividual rdf:about="http://purl.obolibrary.org/obo/GAZ_00142764">
        <obo:RO_0001025 rdf:resource="http://purl.obolibrary.org/obo/GAZ_00016680"/>
        <obo:IAO_0000115>The S cape of Great Barrier Island.</obo:IAO_0000115>
        <oboInOwl:hasOBONamespace>GAZ</oboInOwl:hasOBONamespace>
        <oboInOwl:id>GAZ:00142764</oboInOwl:id>
        <rdfs:label>Cape Barrier</rdfs:label>
    </owl:NamedIndividual>
    


    <!-- http://purl.obolibrary.org/obo/GAZ_00142765 -->

    <owl:NamedIndividual rdf:about="http://purl.obolibrary.org/obo/GAZ_00142765">
        <obo:RO_0001025 rdf:resource="http://purl.obolibrary.org/obo/GAZ_00046945"/>
        <obo:IAO_0000115>One of several passes between the islands of the inner Hauraki Gulf, close to the mouth of the Waitemata Harbour near Auckland city in New Zealand.</obo:IAO_0000115>
        <oboInOwl:hasOBONamespace>GAZ</oboInOwl:hasOBONamespace>
        <oboInOwl:id>GAZ:00142765</oboInOwl:id>
        <rdfs:label>Tamaki Strait</rdfs:label>
    </owl:NamedIndividual>
    


    <!-- http://purl.obolibrary.org/obo/GAZ_00142766 -->

    <owl:NamedIndividual rdf:about="http://purl.obolibrary.org/obo/GAZ_00142766">
        <obo:RO_0001025 rdf:resource="http://purl.obolibrary.org/obo/GAZ_00046945"/>
        <obo:IAO_0000115>A 6 ha island in the Hauraki Gulf of New Zealand.</obo:IAO_0000115>
        <oboInOwl:hasOBONamespace>GAZ</oboInOwl:hasOBONamespace>
        <oboInOwl:id>GAZ:00142766</oboInOwl:id>
        <rdfs:label>Tarahiki Island</rdfs:label>
    </owl:NamedIndividual>
    


    <!-- http://purl.obolibrary.org/obo/GAZ_00142767 -->

    <owl:NamedIndividual rdf:about="http://purl.obolibrary.org/obo/GAZ_00142767">
        <obo:RO_0001025 rdf:resource="http://purl.obolibrary.org/obo/GAZ_00046945"/>
        <obo:IAO_0000115>An island that lies to the west of Great Barrier Island in the Hauraki Gulf in New Zealand. Kaikoura Island is the seventh largest island in the Hauraki Gulf, 90 km north east of Auckland. It forms the natural harbours of Port FitzRoy and Port Abercrombie.</obo:IAO_0000115>
        <oboInOwl:hasOBONamespace>GAZ</oboInOwl:hasOBONamespace>
        <oboInOwl:id>GAZ:00142767</oboInOwl:id>
        <rdfs:label>Kaikoura Island</rdfs:label>
    </owl:NamedIndividual>
    


    <!-- http://purl.obolibrary.org/obo/GAZ_00142768 -->

    <owl:NamedIndividual rdf:about="http://purl.obolibrary.org/obo/GAZ_00142768">
        <obo:RO_0001025 rdf:resource="http://purl.obolibrary.org/obo/GAZ_00046945"/>
        <obo:IAO_0000115>A bay on the W coast of Hauraki Gulf, W of Kawau Island.</obo:IAO_0000115>
        <oboInOwl:hasOBONamespace>GAZ</oboInOwl:hasOBONamespace>
        <oboInOwl:id>GAZ:00142768</oboInOwl:id>
        <rdfs:label>Kawau Bay</rdfs:label>
    </owl:NamedIndividual>
    


    <!-- http://purl.obolibrary.org/obo/GAZ_00142769 -->

    <owl:NamedIndividual rdf:about="http://purl.obolibrary.org/obo/GAZ_00142769">
        <obo:RO_0001025 rdf:resource="http://purl.obolibrary.org/obo/GAZ_00046945"/>
        <obo:IAO_0000115>One of several passes between the islands of the inner Hauraki Gulf, close to the mouth of the Waitemata Harbour to the east of Auckland in New Zealand.</obo:IAO_0000115>
        <oboInOwl:hasOBONamespace>GAZ</oboInOwl:hasOBONamespace>
        <oboInOwl:id>GAZ:00142769</oboInOwl:id>
        <rdfs:label>Rangitoto Channel</rdfs:label>
    </owl:NamedIndividual>
    


    <!-- http://purl.obolibrary.org/obo/GAZ_00142770 -->

    <owl:NamedIndividual rdf:about="http://purl.obolibrary.org/obo/GAZ_00142770">
        <obo:RO_0001025 rdf:resource="http://purl.obolibrary.org/obo/GAZ_00046945"/>
        <obo:IAO_0000115>A large bay located in the north of the North Island of New Zealand. It is the firth of the rivers Waihou and Piako. The firth lies at the southern end of the Hauraki Gulf, southeast of the city of Auckland. It occupies a rift valley or graben between the Coromandel Peninsula and Hunua Ranges which continues into the Hauraki Plains to the south. The S of the Bay is a Ramsar Site.</obo:IAO_0000115>
        <oboInOwl:hasOBONamespace>GAZ</oboInOwl:hasOBONamespace>
        <oboInOwl:id>GAZ:00142770</oboInOwl:id>
        <rdfs:label>Firth of Thames</rdfs:label>
    </owl:NamedIndividual>
    


    <!-- http://purl.obolibrary.org/obo/GAZ_00142771 -->

    <owl:NamedIndividual rdf:about="http://purl.obolibrary.org/obo/GAZ_00142771">
        <obo:RO_0001025 rdf:resource="http://purl.obolibrary.org/obo/GAZ_00046945"/>
        <obo:IAO_0000115>A tiny island (approximately 1 ha) located close to the North Island coast northeast of Warkworth, and directly west of Hauturu/Little Barrier Island.</obo:IAO_0000115>
        <oboInOwl:hasOBONamespace>GAZ</oboInOwl:hasOBONamespace>
        <oboInOwl:id>GAZ:00142771</oboInOwl:id>
        <rdfs:label>Goat Island</rdfs:label>
    </owl:NamedIndividual>
    


    <!-- http://purl.obolibrary.org/obo/GAZ_00142772 -->

    <owl:NamedIndividual rdf:about="http://purl.obolibrary.org/obo/GAZ_00142772">
        <rdf:type rdf:resource="http://purl.obolibrary.org/obo/ENVO_00000475"/>
        <obo:RO_0001025 rdf:resource="http://purl.obolibrary.org/obo/GAZ_00004760"/>
        <obo:RO_0001025 rdf:resource="http://purl.obolibrary.org/obo/GAZ_00046945"/>
        <obo:IAO_0000115>An arm of the Hauraki Gulf, extending west for eighteen km from the end of the Rangitoto Channel. Its entrance is between North Head and Bastion Point in the south. The westernmost ends of the harbour extend past Whenuapai in the northwest, and to Te Atatu in the west, as well as forming the estuarial arm known as the Whau River in the southwest. The harbour is a drowned valley system in marine sediments deposited during the Miocene.</obo:IAO_0000115>
        <oboInOwl:hasOBONamespace>GAZ</oboInOwl:hasOBONamespace>
        <oboInOwl:id>GAZ:00142772</oboInOwl:id>
        <rdfs:label>Waitemata Harbour</rdfs:label>
    </owl:NamedIndividual>
    


    <!-- http://purl.obolibrary.org/obo/GAZ_00142773 -->

    <owl:NamedIndividual rdf:about="http://purl.obolibrary.org/obo/GAZ_00142773">
        <obo:RO_0001025 rdf:resource="http://purl.obolibrary.org/obo/GAZ_00046945"/>
        <obo:IAO_0000115>One of three channels connecting the Hauraki Gulf with the Pacific Ocean to the northeast of Auckland, New Zealand. It is the westernmost channel, lying between Cape Rodney on the North Auckland Peninsula and Hauturu/Little Barrier Island.</obo:IAO_0000115>
        <oboInOwl:hasOBONamespace>GAZ</oboInOwl:hasOBONamespace>
        <oboInOwl:id>GAZ:00142773</oboInOwl:id>
        <rdfs:label>Jellicoe Channel</rdfs:label>
    </owl:NamedIndividual>
    


    <!-- http://purl.obolibrary.org/obo/GAZ_00142774 -->

    <owl:NamedIndividual rdf:about="http://purl.obolibrary.org/obo/GAZ_00142774">
        <obo:RO_0001025 rdf:resource="http://purl.obolibrary.org/obo/GAZ_00046945"/>
        <obo:IAO_0000115>An island that lies between Motutapu and Waiheke islands in the Hauraki Gulf of New Zealand, close to the Auckland area.</obo:IAO_0000115>
        <oboInOwl:hasOBONamespace>GAZ</oboInOwl:hasOBONamespace>
        <oboInOwl:id>GAZ:00142774</oboInOwl:id>
        <rdfs:label>Motuihe Island</rdfs:label>
    </owl:NamedIndividual>
    


    <!-- http://purl.obolibrary.org/obo/GAZ_00142775 -->

    <owl:NamedIndividual rdf:about="http://purl.obolibrary.org/obo/GAZ_00142775">
        <obo:RO_0001025 rdf:resource="http://purl.obolibrary.org/obo/GAZ_00142772"/>
        <obo:IAO_0000115>An n estuarial arm of the southwestern Waitemata Harbour (not a river), within the Auckland metropolitan area in New Zealand. It extends south for five km from its mouth between the Te Atatu peninsula and the long thin Rosebank Peninsula in Avondale.</obo:IAO_0000115>
        <oboInOwl:hasOBONamespace>GAZ</oboInOwl:hasOBONamespace>
        <oboInOwl:id>GAZ:00142775</oboInOwl:id>
        <rdfs:label>Whau River</rdfs:label>
    </owl:NamedIndividual>
    


    <!-- http://purl.obolibrary.org/obo/GAZ_00142776 -->

    <owl:NamedIndividual rdf:about="http://purl.obolibrary.org/obo/GAZ_00142776">
        <obo:RO_0001025 rdf:resource="http://purl.obolibrary.org/obo/GAZ_00142772"/>
        <obo:IAO_0000115>A small island.</obo:IAO_0000115>
        <oboInOwl:hasOBONamespace>GAZ</oboInOwl:hasOBONamespace>
        <oboInOwl:id>GAZ:00142776</oboInOwl:id>
        <rdfs:label>Pollen Island</rdfs:label>
    </owl:NamedIndividual>
    


    <!-- http://purl.obolibrary.org/obo/GAZ_00142777 -->

    <owl:NamedIndividual rdf:about="http://purl.obolibrary.org/obo/GAZ_00142777">
        <obo:RO_0001025 rdf:resource="http://purl.obolibrary.org/obo/GAZ_00142772"/>
        <obo:IAO_0000115>A small island.</obo:IAO_0000115>
        <oboInOwl:hasOBONamespace>GAZ</oboInOwl:hasOBONamespace>
        <oboInOwl:id>GAZ:00142777</oboInOwl:id>
        <rdfs:label>Traherne Island</rdfs:label>
    </owl:NamedIndividual>
    


    <!-- http://purl.obolibrary.org/obo/GAZ_00142778 -->

    <owl:NamedIndividual rdf:about="http://purl.obolibrary.org/obo/GAZ_00142778">
        <obo:RO_0001025 rdf:resource="http://purl.obolibrary.org/obo/GAZ_00142776"/>
        <obo:IAO_0000115>A protected area.</obo:IAO_0000115>
        <oboInOwl:hasOBONamespace>GAZ</oboInOwl:hasOBONamespace>
        <oboInOwl:id>GAZ:00142778</oboInOwl:id>
        <rdfs:label>Motu Manawa/Pollen Island Marine Reserve</rdfs:label>
    </owl:NamedIndividual>
    


    <!-- http://purl.obolibrary.org/obo/GAZ_00142780 -->

    <owl:NamedIndividual rdf:about="http://purl.obolibrary.org/obo/GAZ_00142780">
        <rdf:type rdf:resource="http://purl.obolibrary.org/obo/ENVO_00000222"/>
        <obo:RO_0001025 rdf:resource="http://purl.obolibrary.org/obo/GAZ_00142875"/>
        <obo:IAO_0000115>A volcanic island in the Manukau Harbour, New Zealand, and is part of the Auckland volcanic field.</obo:IAO_0000115>
        <oboInOwl:hasOBONamespace>GAZ</oboInOwl:hasOBONamespace>
        <oboInOwl:id>GAZ:00142780</oboInOwl:id>
        <rdfs:label>Puketutu Island</rdfs:label>
    </owl:NamedIndividual>
    


    <!-- http://purl.obolibrary.org/obo/GAZ_00142781 -->

    <owl:NamedIndividual rdf:about="http://purl.obolibrary.org/obo/GAZ_00142781">
        <obo:RO_0001025 rdf:resource="http://purl.obolibrary.org/obo/GAZ_00142772"/>
        <obo:IAO_0000115>A small sandstone island in the Waitemata Harbour of Auckland, New Zealand. It lies approximately one km north of the Herne Bay suburb.</obo:IAO_0000115>
        <oboInOwl:hasOBONamespace>GAZ</oboInOwl:hasOBONamespace>
        <oboInOwl:id>GAZ:00142781</oboInOwl:id>
        <rdfs:label>Watchman Island</rdfs:label>
    </owl:NamedIndividual>
    


    <!-- http://purl.obolibrary.org/obo/GAZ_00142782 -->

    <owl:NamedIndividual rdf:about="http://purl.obolibrary.org/obo/GAZ_00142782">
        <obo:RO_0001025 rdf:resource="http://purl.obolibrary.org/obo/GAZ_00016691"/>
        <obo:IAO_0000115>The NE point of Waiheke Island.</obo:IAO_0000115>
        <oboInOwl:hasOBONamespace>GAZ</oboInOwl:hasOBONamespace>
        <oboInOwl:id>GAZ:00142782</oboInOwl:id>
        <rdfs:label>Thumb Point</rdfs:label>
    </owl:NamedIndividual>
    


    <!-- http://purl.obolibrary.org/obo/GAZ_00142784 -->

    <owl:NamedIndividual rdf:about="http://purl.obolibrary.org/obo/GAZ_00142784">
        <obo:RO_0001025 rdf:resource="http://purl.obolibrary.org/obo/GAZ_00046945"/>
        <obo:IAO_0000115>A bay in the NW coast of Hauraki Gulf.</obo:IAO_0000115>
        <oboInOwl:hasOBONamespace>GAZ</oboInOwl:hasOBONamespace>
        <oboInOwl:id>GAZ:00142784</oboInOwl:id>
        <rdfs:label>Mangawhai Harbour</rdfs:label>
    </owl:NamedIndividual>
    


    <!-- http://purl.obolibrary.org/obo/GAZ_00142799 -->

    <owl:NamedIndividual rdf:about="http://purl.obolibrary.org/obo/GAZ_00142799">
        <obo:RO_0001025 rdf:resource="http://purl.obolibrary.org/obo/GAZ_00046945"/>
        <obo:IAO_0000115>An island just N of Cape Rodney.</obo:IAO_0000115>
        <oboInOwl:hasOBONamespace>GAZ</oboInOwl:hasOBONamespace>
        <oboInOwl:id>GAZ:00142799</oboInOwl:id>
        <rdfs:label>Goat Island</rdfs:label>
    </owl:NamedIndividual>
    


    <!-- http://purl.obolibrary.org/obo/GAZ_00142800 -->

    <owl:NamedIndividual rdf:about="http://purl.obolibrary.org/obo/GAZ_00142800">
        <obo:RO_0001025 rdf:resource="http://purl.obolibrary.org/obo/GAZ_00046945"/>
        <obo:IAO_0000115>A small island to the SW of Kawau Island.</obo:IAO_0000115>
        <oboInOwl:hasOBONamespace>GAZ</oboInOwl:hasOBONamespace>
        <oboInOwl:id>GAZ:00142800</oboInOwl:id>
        <rdfs:label>Motutara Island</rdfs:label>
    </owl:NamedIndividual>
    


    <!-- http://purl.obolibrary.org/obo/GAZ_00142801 -->

    <owl:NamedIndividual rdf:about="http://purl.obolibrary.org/obo/GAZ_00142801">
        <obo:RO_0001025 rdf:resource="http://purl.obolibrary.org/obo/GAZ_00046945"/>
        <obo:IAO_0000115>A small island to the SW of Kawau Island.</obo:IAO_0000115>
        <oboInOwl:hasOBONamespace>GAZ</oboInOwl:hasOBONamespace>
        <oboInOwl:id>GAZ:00142801</oboInOwl:id>
        <rdfs:label>Beehive Island</rdfs:label>
    </owl:NamedIndividual>
    


    <!-- http://purl.obolibrary.org/obo/GAZ_00142802 -->

    <owl:NamedIndividual rdf:about="http://purl.obolibrary.org/obo/GAZ_00142802">
        <obo:RO_0001025 rdf:resource="http://purl.obolibrary.org/obo/GAZ_00046945"/>
        <obo:IAO_0000115>A small island to the SW of Kawau Island.</obo:IAO_0000115>
        <oboInOwl:hasOBONamespace>GAZ</oboInOwl:hasOBONamespace>
        <oboInOwl:id>GAZ:00142802</oboInOwl:id>
        <rdfs:label>Motuora Island</rdfs:label>
    </owl:NamedIndividual>
    


    <!-- http://purl.obolibrary.org/obo/GAZ_00142803 -->

    <owl:NamedIndividual rdf:about="http://purl.obolibrary.org/obo/GAZ_00142803">
        <obo:RO_0001025 rdf:resource="http://purl.obolibrary.org/obo/GAZ_00046945"/>
        <obo:IAO_0000115>A small island to the SW of Kawau Island.</obo:IAO_0000115>
        <oboInOwl:hasOBONamespace>GAZ</oboInOwl:hasOBONamespace>
        <oboInOwl:id>GAZ:00142803</oboInOwl:id>
        <rdfs:label>Kobatutara Island</rdfs:label>
    </owl:NamedIndividual>
    


    <!-- http://purl.obolibrary.org/obo/GAZ_00142804 -->

    <owl:NamedIndividual rdf:about="http://purl.obolibrary.org/obo/GAZ_00142804">
        <obo:RO_0001025 rdf:resource="http://purl.obolibrary.org/obo/GAZ_00046945"/>
        <obo:IAO_0000115>A small island to the SW of Kawau Island.</obo:IAO_0000115>
        <oboInOwl:hasOBONamespace>GAZ</oboInOwl:hasOBONamespace>
        <oboInOwl:id>GAZ:00142804</oboInOwl:id>
        <rdfs:label>Moturekareka Island</rdfs:label>
    </owl:NamedIndividual>
    


    <!-- http://purl.obolibrary.org/obo/GAZ_00142839 -->

    <owl:NamedIndividual rdf:about="http://purl.obolibrary.org/obo/GAZ_00142839">
        <obo:RO_0001025 rdf:resource="http://purl.obolibrary.org/obo/GAZ_00029928"/>
        <obo:IAO_0000115>A tombolo at the northern tip of the North Island of New Zealand. It projects between the Tasman Sea to the west and the Pacific Ocean to the east. It constitutes the northern part of the Far North District, consisting of the area North Cape, Houhora and the northern half of Awanui.</obo:IAO_0000115>
        <oboInOwl:hasOBONamespace>GAZ</oboInOwl:hasOBONamespace>
        <oboInOwl:id>GAZ:00142839</oboInOwl:id>
        <rdfs:label>Aupouri Peninsula</rdfs:label>
    </owl:NamedIndividual>
    


    <!-- http://purl.obolibrary.org/obo/GAZ_00142840 -->

    <owl:NamedIndividual rdf:about="http://purl.obolibrary.org/obo/GAZ_00142840">
        <obo:RO_0001025 rdf:resource="http://purl.obolibrary.org/obo/GAZ_00142839"/>
        <obo:IAO_0000115>The westernmost point of the North Island of New Zealand. Being close to the northern tip of the Aupouri Peninsula.</obo:IAO_0000115>
        <oboInOwl:hasOBONamespace>GAZ</oboInOwl:hasOBONamespace>
        <oboInOwl:id>GAZ:00142840</oboInOwl:id>
        <rdfs:label>Cape Maria van Diemen</rdfs:label>
    </owl:NamedIndividual>
    


    <!-- http://purl.obolibrary.org/obo/GAZ_00142841 -->

    <owl:NamedIndividual rdf:about="http://purl.obolibrary.org/obo/GAZ_00142841">
        <obo:RO_0001025 rdf:resource="http://purl.obolibrary.org/obo/GAZ_00142842"/>
        <obo:IAO_0000115>The northernmost point of the mainland of New Zealand. They are situated on the North Cape of the North Island, 30 km to the east of Cape Reinga.</obo:IAO_0000115>
        <oboInOwl:hasOBONamespace>GAZ</oboInOwl:hasOBONamespace>
        <oboInOwl:id>GAZ:00142841</oboInOwl:id>
        <rdfs:label>Surville Cliffs</rdfs:label>
    </owl:NamedIndividual>
    


    <!-- http://purl.obolibrary.org/obo/GAZ_00142842 -->

    <owl:NamedIndividual rdf:about="http://purl.obolibrary.org/obo/GAZ_00142842">
        <obo:RO_0001025 rdf:resource="http://purl.obolibrary.org/obo/GAZ_00142839"/>
        <obo:IAO_0000115>A capeat the northern end of the North Auckland Peninsula in the North Island of New Zealand. It is the northeastern tip of the Aupouri Peninsula and lies 30 km east of Cape Reinga.</obo:IAO_0000115>
        <oboInOwl:hasOBONamespace>GAZ</oboInOwl:hasOBONamespace>
        <oboInOwl:id>GAZ:00142842</oboInOwl:id>
        <rdfs:label>North Cape</rdfs:label>
    </owl:NamedIndividual>
    


    <!-- http://purl.obolibrary.org/obo/GAZ_00142843 -->

    <owl:NamedIndividual rdf:about="http://purl.obolibrary.org/obo/GAZ_00142843">
        <obo:RO_0001025 rdf:resource="http://purl.obolibrary.org/obo/GAZ_00142839"/>
        <obo:IAO_0000115>The northwesternmost tip of the Aupouri Peninsula, at the northern end of the North Island of New Zealand. Cape Reinga is located over 100 km north of the nearest small town of Kaitaia. Cape Reinga is generally considered the separation marker between the Tasman Sea to the west and the Pacific Ocean to the east.</obo:IAO_0000115>
        <oboInOwl:hasOBONamespace>GAZ</oboInOwl:hasOBONamespace>
        <oboInOwl:id>GAZ:00142843</oboInOwl:id>
        <rdfs:label>Cape Reinga</rdfs:label>
    </owl:NamedIndividual>
    


    <!-- http://purl.obolibrary.org/obo/GAZ_00142846 -->

    <owl:NamedIndividual rdf:about="http://purl.obolibrary.org/obo/GAZ_00142846">
        <obo:RO_0001025 rdf:resource="http://purl.obolibrary.org/obo/GAZ_00004760"/>
        <obo:RO_0001025 rdf:resource="http://purl.obolibrary.org/obo/GAZ_00008569"/>
        <obo:IAO_0000115>The major peninsula to the N of Auckland on North Island. Terminates in the Aupouri Peninsula.</obo:IAO_0000115>
        <oboInOwl:hasOBONamespace>GAZ</oboInOwl:hasOBONamespace>
        <oboInOwl:id>GAZ:00142846</oboInOwl:id>
        <rdfs:label>North Auckland Peninsula</rdfs:label>
    </owl:NamedIndividual>
    


    <!-- http://purl.obolibrary.org/obo/GAZ_00142847 -->

    <owl:NamedIndividual rdf:about="http://purl.obolibrary.org/obo/GAZ_00142847">
        <obo:RO_0001025 rdf:resource="http://purl.obolibrary.org/obo/GAZ_00142846"/>
        <obo:IAO_0000115>A rocky land mass, originally an island, which is joined to the Aupouri Peninsula in Northland, New Zealand by a low sandy strip about 13 km long. Rangaunu Bay is to the west and Doubtless Bay is to the southeast. The Moturoa Islands are to the northwest. Rangaunu Harbour and Tokerau Beach are on the west and east sides of the strip.</obo:IAO_0000115>
        <oboInOwl:hasOBONamespace>GAZ</oboInOwl:hasOBONamespace>
        <oboInOwl:id>GAZ:00142847</oboInOwl:id>
        <rdfs:label>Karikari Peninsula</rdfs:label>
    </owl:NamedIndividual>
    


    <!-- http://purl.obolibrary.org/obo/GAZ_00142869 -->

    <owl:NamedIndividual rdf:about="http://purl.obolibrary.org/obo/GAZ_00142869">
        <obo:RO_0001025 rdf:resource="http://purl.obolibrary.org/obo/GAZ_00029928"/>
        <obo:IAO_0000115>An island just off Cape Maria van Diemen.</obo:IAO_0000115>
        <oboInOwl:hasOBONamespace>GAZ</oboInOwl:hasOBONamespace>
        <oboInOwl:id>GAZ:00142869</oboInOwl:id>
        <rdfs:label>Motuopao Island</rdfs:label>
    </owl:NamedIndividual>
    


    <!-- http://purl.obolibrary.org/obo/GAZ_00142871 -->

    <owl:NamedIndividual rdf:about="http://purl.obolibrary.org/obo/GAZ_00142871">
        <obo:RO_0001025 rdf:resource="http://purl.obolibrary.org/obo/GAZ_00004765"/>
        <obo:IAO_0000115>The southernmost part of Ninety Mile Beach, a beach located on the western coast of the far north of the North Island of New Zealand. It stretches from just west of Kaitaia towards Cape Reinga along the Aupouri Peninsula. It begins close to the headland of Reef Point, to the west of Ahipara Bay, sweeping briefly northeast before turning northwest for the majority of its length. It ends at Scott Point, five km south of Cape Maria van Diemen.</obo:IAO_0000115>
        <oboInOwl:hasOBONamespace>GAZ</oboInOwl:hasOBONamespace>
        <oboInOwl:id>GAZ:00142871</oboInOwl:id>
        <rdfs:label>Ahipara Bay</rdfs:label>
    </owl:NamedIndividual>
    


    <!-- http://purl.obolibrary.org/obo/GAZ_00142875 -->

    <owl:NamedIndividual rdf:about="http://purl.obolibrary.org/obo/GAZ_00142875">
        <obo:RO_0001025 rdf:resource="http://purl.obolibrary.org/obo/GAZ_00000469"/>
        <obo:RO_0001025 rdf:resource="http://purl.obolibrary.org/obo/GAZ_00004760"/>
        <obo:IAO_0000115>A harbor located to the southwest of the Auckland isthmus, and is an arm of the Tasman Sea. The harbour mouth is between the northern head (Burnett Head / Ohaka Head) located at the southern end of the Waitakere Ranges and South Head at the end of the long Awhitu Peninsula reaching up from close to the mouth of the Waikato River. The mouth is only 1800 metres wide, but after a 9 km channel it opens up into a roughly square basin 20 km in width.</obo:IAO_0000115>
        <oboInOwl:hasOBONamespace>GAZ</oboInOwl:hasOBONamespace>
        <oboInOwl:id>GAZ:00142875</oboInOwl:id>
        <rdfs:label>Manukau Harbor</rdfs:label>
    </owl:NamedIndividual>
    


    <!-- http://purl.obolibrary.org/obo/GAZ_00142876 -->

    <owl:NamedIndividual rdf:about="http://purl.obolibrary.org/obo/GAZ_00142876">
        <rdf:type rdf:resource="http://purl.obolibrary.org/obo/ENVO_00000475"/>
        <obo:RO_0001025 rdf:resource="http://purl.obolibrary.org/obo/GAZ_00142875"/>
        <obo:IAO_0000115>An arm of Manukau Harbour.</obo:IAO_0000115>
        <oboInOwl:hasOBONamespace>GAZ</oboInOwl:hasOBONamespace>
        <oboInOwl:id>GAZ:00142876</oboInOwl:id>
        <rdfs:label>Papakura Channel</rdfs:label>
    </owl:NamedIndividual>
    


    <!-- http://purl.obolibrary.org/obo/GAZ_00142877 -->

    <owl:NamedIndividual rdf:about="http://purl.obolibrary.org/obo/GAZ_00142877">
        <rdf:type rdf:resource="http://purl.obolibrary.org/obo/ENVO_00000475"/>
        <obo:RO_0001025 rdf:resource="http://purl.obolibrary.org/obo/GAZ_00142875"/>
        <obo:IAO_0000115>An arm of Manukau Harbour.</obo:IAO_0000115>
        <oboInOwl:hasOBONamespace>GAZ</oboInOwl:hasOBONamespace>
        <oboInOwl:id>GAZ:00142877</oboInOwl:id>
        <rdfs:label>Mangere Inlet</rdfs:label>
    </owl:NamedIndividual>
    


    <!-- http://purl.obolibrary.org/obo/GAZ_00142878 -->

    <owl:NamedIndividual rdf:about="http://purl.obolibrary.org/obo/GAZ_00142878">
        <obo:RO_0001025 rdf:resource="http://purl.obolibrary.org/obo/GAZ_00142875"/>
        <obo:IAO_0000115>An estuarial arm of Manukau Harbor (not a river). It is s located to the southwest of the city of Auckland in New Zealand.</obo:IAO_0000115>
        <oboInOwl:hasOBONamespace>GAZ</oboInOwl:hasOBONamespace>
        <oboInOwl:id>GAZ:00142878</oboInOwl:id>
        <rdfs:label>Waiuku River</rdfs:label>
    </owl:NamedIndividual>
    


    <!-- http://purl.obolibrary.org/obo/GAZ_00144841 -->

    <owl:NamedIndividual rdf:about="http://purl.obolibrary.org/obo/GAZ_00144841">
        <obo:RO_0001025 rdf:resource="http://purl.obolibrary.org/obo/GAZ_00053293"/>
        <obo:IAO_0000115>A highly dynamic acid crater lake.</obo:IAO_0000115>
        <oboInOwl:hasOBONamespace>GAZ</oboInOwl:hasOBONamespace>
        <oboInOwl:id>GAZ:00144841</oboInOwl:id>
        <rdfs:label>Mount Ruapehu Crater Lake</rdfs:label>
    </owl:NamedIndividual>
    


    <!-- http://purl.obolibrary.org/obo/GAZ_00146174 -->

    <owl:NamedIndividual rdf:about="http://purl.obolibrary.org/obo/GAZ_00146174">
        <obo:RO_0001025 rdf:resource="http://purl.obolibrary.org/obo/GAZ_00007723"/>
        <obo:IAO_0000115>A peninsula that lies in the North Island of New Zealand. It is part of the Waikato region and extends 85 km north from the western end of the Bay of Plenty, forming a natural barrier to protect the Hauraki Gulf and the Firth of Thames in the west from the Pacific Ocean to the east.</obo:IAO_0000115>
        <oboInOwl:hasOBONamespace>GAZ</oboInOwl:hasOBONamespace>
        <oboInOwl:id>GAZ:00146174</oboInOwl:id>
        <rdfs:label>Coromandel Peninsula</rdfs:label>
    </owl:NamedIndividual>
    


    <!-- http://purl.obolibrary.org/obo/GAZ_00146175 -->

    <owl:NamedIndividual rdf:about="http://purl.obolibrary.org/obo/GAZ_00146175">
        <obo:RO_0001025 rdf:resource="http://purl.obolibrary.org/obo/GAZ_00146174"/>
        <obo:IAO_0000115>A ridge of rugged hills running the length of the Coromandel Peninsula in the North Island of New Zealand. It is located 60 km east of the city of Auckland, and runs north-south for approximately 85 km.</obo:IAO_0000115>
        <oboInOwl:hasOBONamespace>GAZ</oboInOwl:hasOBONamespace>
        <oboInOwl:id>GAZ:00146175</oboInOwl:id>
        <rdfs:label>Coromandel Range</rdfs:label>
    </owl:NamedIndividual>
    


    <!-- http://purl.obolibrary.org/obo/GAZ_00146176 -->

    <owl:NamedIndividual rdf:about="http://purl.obolibrary.org/obo/GAZ_00146176">
        <obo:RO_0001025 rdf:resource="http://purl.obolibrary.org/obo/GAZ_00146174"/>
        <obo:IAO_0000115>The northernmost range on the Coromandel Peninsula, extending from the settlement of Colville northwards to the tip of the peninsula.</obo:IAO_0000115>
        <oboInOwl:hasOBONamespace>GAZ</oboInOwl:hasOBONamespace>
        <oboInOwl:id>GAZ:00146176</oboInOwl:id>
        <rdfs:label>Moehau Range</rdfs:label>
    </owl:NamedIndividual>
    


    <!-- http://purl.obolibrary.org/obo/GAZ_00146177 -->

    <owl:NamedIndividual rdf:about="http://purl.obolibrary.org/obo/GAZ_00146177">
        <obo:RO_0001025 rdf:resource="http://purl.obolibrary.org/obo/GAZ_00004765"/>
        <obo:IAO_0000115>A mountain range in the North Island of New Zealand. It can be seen as a continuation southwards of the hills of the Coromandel Peninsula, and separates the Waikato in the west from the Bay of Plenty in the east.</obo:IAO_0000115>
        <oboInOwl:hasOBONamespace>GAZ</oboInOwl:hasOBONamespace>
        <oboInOwl:id>GAZ:00146177</oboInOwl:id>
        <rdfs:label>Kaimai Ranges</rdfs:label>
    </owl:NamedIndividual>
    


    <!-- http://purl.obolibrary.org/obo/GAZ_00146178 -->

    <owl:NamedIndividual rdf:about="http://purl.obolibrary.org/obo/GAZ_00146178">
        <obo:RO_0001025 rdf:resource="http://purl.obolibrary.org/obo/GAZ_00146174"/>
        <obo:IAO_0000115>A beach on the east coast of the Coromandel Peninsula, New Zealand, approximately 12 km south east of Whitianga. Its name comes from underground hot springs which filter up through the sand between the high and low water tidal reaches.</obo:IAO_0000115>
        <oboInOwl:hasOBONamespace>GAZ</oboInOwl:hasOBONamespace>
        <oboInOwl:id>GAZ:00146178</oboInOwl:id>
        <rdfs:label>Hot Water Beach</rdfs:label>
    </owl:NamedIndividual>
    


    <!-- http://purl.obolibrary.org/obo/GAZ_00146179 -->

    <owl:NamedIndividual rdf:about="http://purl.obolibrary.org/obo/GAZ_00146179">
        <obo:RO_0001025 rdf:resource="http://purl.obolibrary.org/obo/GAZ_00146178"/>
        <obo:IAO_0000115>Hot springs under Hot Water Beach.</obo:IAO_0000115>
        <oboInOwl:hasOBONamespace>GAZ</oboInOwl:hasOBONamespace>
        <oboInOwl:id>GAZ:00146179</oboInOwl:id>
        <rdfs:label>Hot Water Springs</rdfs:label>
    </owl:NamedIndividual>
    


    <!-- http://purl.obolibrary.org/obo/GAZ_00146180 -->

    <owl:NamedIndividual rdf:about="http://purl.obolibrary.org/obo/GAZ_00146180">
        <rdf:type rdf:resource="http://purl.obolibrary.org/obo/ENVO_00000856"/>
        <obo:RO_0001025 rdf:resource="http://purl.obolibrary.org/obo/GAZ_00029928"/>
    </owl:NamedIndividual>
    


    <!-- http://purl.obolibrary.org/obo/GAZ_00146181 -->

    <owl:NamedIndividual rdf:about="http://purl.obolibrary.org/obo/GAZ_00146181">
        <rdf:type rdf:resource="http://purl.obolibrary.org/obo/ENVO_00000062"/>
        <obo:RO_0001025 rdf:resource="http://purl.obolibrary.org/obo/GAZ_00029928"/>
    </owl:NamedIndividual>
    


    <!-- http://purl.obolibrary.org/obo/GAZ_00146182 -->

    <owl:NamedIndividual rdf:about="http://purl.obolibrary.org/obo/GAZ_00146182">
        <obo:RO_0001025 rdf:resource="http://purl.obolibrary.org/obo/GAZ_00053832"/>
        <obo:RO_0001025 rdf:resource="http://purl.obolibrary.org/obo/GAZ_00146181"/>
        <obo:IAO_0000115>Hot springs.</obo:IAO_0000115>
        <oboInOwl:hasOBONamespace>GAZ</oboInOwl:hasOBONamespace>
        <oboInOwl:id>GAZ:00146182</oboInOwl:id>
        <rdfs:label>Ngawha Springs</rdfs:label>
    </owl:NamedIndividual>
    


    <!-- http://purl.obolibrary.org/obo/GAZ_00146183 -->

    <owl:NamedIndividual rdf:about="http://purl.obolibrary.org/obo/GAZ_00146183">
        <obo:RO_0001025 rdf:resource="http://purl.obolibrary.org/obo/GAZ_00053854"/>
        <obo:IAO_0000115>A sinter terrace.</obo:IAO_0000115>
        <oboInOwl:hasOBONamespace>GAZ</oboInOwl:hasOBONamespace>
        <oboInOwl:id>GAZ:00146183</oboInOwl:id>
        <rdfs:label>Emerald Terrace</rdfs:label>
    </owl:NamedIndividual>
    


    <!-- http://purl.obolibrary.org/obo/GAZ_00146184 -->

    <owl:NamedIndividual rdf:about="http://purl.obolibrary.org/obo/GAZ_00146184">
        <obo:RO_0001025 rdf:resource="http://purl.obolibrary.org/obo/GAZ_00053854"/>
        <obo:IAO_0000115>An artificial lake that drowned many geysers and hot springs ar Orakei Korako. Resulting from a hydroelectric dam on the Waikato River. Completed 1961.</obo:IAO_0000115>
        <oboInOwl:hasOBONamespace>GAZ</oboInOwl:hasOBONamespace>
        <oboInOwl:id>GAZ:00146184</oboInOwl:id>
        <rdfs:label>Lake Ohakuri</rdfs:label>
    </owl:NamedIndividual>
    


    <!-- http://purl.obolibrary.org/obo/GAZ_00146185 -->

    <owl:NamedIndividual rdf:about="http://purl.obolibrary.org/obo/GAZ_00146185">
        <obo:RO_0001025 rdf:resource="http://purl.obolibrary.org/obo/GAZ_00053854"/>
        <obo:IAO_0000115>A former geyser drowned under Lake Ohakuri.</obo:IAO_0000115>
        <oboInOwl:hasOBONamespace>GAZ</oboInOwl:hasOBONamespace>
        <oboInOwl:id>GAZ:00146185</oboInOwl:id>
        <rdfs:label>Orakeikorako Geyser</rdfs:label>
    </owl:NamedIndividual>
    


    <!-- http://purl.obolibrary.org/obo/GAZ_00146186 -->

    <owl:NamedIndividual rdf:about="http://purl.obolibrary.org/obo/GAZ_00146186">
        <obo:RO_0001025 rdf:resource="http://purl.obolibrary.org/obo/GAZ_00053854"/>
        <obo:IAO_0000115>A former geyser drowned under Lake Ohakuri.</obo:IAO_0000115>
        <oboInOwl:hasOBONamespace>GAZ</oboInOwl:hasOBONamespace>
        <oboInOwl:id>GAZ:00146186</oboInOwl:id>
        <rdfs:label>Minginui Geyser</rdfs:label>
    </owl:NamedIndividual>
    


    <!-- http://purl.obolibrary.org/obo/GAZ_00146187 -->

    <owl:NamedIndividual rdf:about="http://purl.obolibrary.org/obo/GAZ_00146187">
        <obo:RO_0001025 rdf:resource="http://purl.obolibrary.org/obo/GAZ_00053854"/>
        <obo:IAO_0000115>An active geyser.</obo:IAO_0000115>
        <oboInOwl:hasOBONamespace>GAZ</oboInOwl:hasOBONamespace>
        <oboInOwl:id>GAZ:00146187</oboInOwl:id>
        <rdfs:label>Diamond Geyser</rdfs:label>
    </owl:NamedIndividual>
    


    <!-- http://purl.obolibrary.org/obo/GAZ_00146188 -->

    <owl:NamedIndividual rdf:about="http://purl.obolibrary.org/obo/GAZ_00146188">
        <obo:RO_0001025 rdf:resource="http://purl.obolibrary.org/obo/GAZ_00053854"/>
        <obo:IAO_0000115>A sinter terrace.</obo:IAO_0000115>
        <oboInOwl:hasOBONamespace>GAZ</oboInOwl:hasOBONamespace>
        <oboInOwl:id>GAZ:00146188</oboInOwl:id>
        <rdfs:label>Rainbow Terrace</rdfs:label>
    </owl:NamedIndividual>
    


    <!-- http://purl.obolibrary.org/obo/GAZ_00146189 -->

    <owl:NamedIndividual rdf:about="http://purl.obolibrary.org/obo/GAZ_00146189">
        <obo:RO_0001025 rdf:resource="http://purl.obolibrary.org/obo/GAZ_00053854"/>
        <obo:IAO_0000115>A sinter terrace.</obo:IAO_0000115>
        <oboInOwl:hasOBONamespace>GAZ</oboInOwl:hasOBONamespace>
        <oboInOwl:id>GAZ:00146189</oboInOwl:id>
        <rdfs:label>Cascade Terrace</rdfs:label>
    </owl:NamedIndividual>
    


    <!-- http://purl.obolibrary.org/obo/GAZ_00146190 -->

    <owl:NamedIndividual rdf:about="http://purl.obolibrary.org/obo/GAZ_00146190">
        <obo:RO_0001025 rdf:resource="http://purl.obolibrary.org/obo/GAZ_00053854"/>
        <obo:IAO_0000115>An intermittently active geyser.</obo:IAO_0000115>
        <oboInOwl:hasOBONamespace>GAZ</oboInOwl:hasOBONamespace>
        <oboInOwl:id>GAZ:00146190</oboInOwl:id>
        <rdfs:label>Sapphire Geyser</rdfs:label>
    </owl:NamedIndividual>
    


    <!-- http://purl.obolibrary.org/obo/GAZ_00146191 -->

    <owl:NamedIndividual rdf:about="http://purl.obolibrary.org/obo/GAZ_00146191">
        <obo:RO_0001025 rdf:resource="http://purl.obolibrary.org/obo/GAZ_00053854"/>
        <obo:IAO_0000115>A former geyser. It erupted in 1954-11 and played as a geyser until mid-1955, ceasing suddenly after swarms of subterranean earthquakes.</obo:IAO_0000115>
        <oboInOwl:hasOBONamespace>GAZ</oboInOwl:hasOBONamespace>
        <oboInOwl:id>GAZ:00146191</oboInOwl:id>
        <rdfs:label>Hochstetter Pool</rdfs:label>
    </owl:NamedIndividual>
    


    <!-- http://purl.obolibrary.org/obo/GAZ_00146192 -->

    <owl:NamedIndividual rdf:about="http://purl.obolibrary.org/obo/GAZ_00146192">
        <obo:RO_0001025 rdf:resource="http://purl.obolibrary.org/obo/GAZ_00053854"/>
        <obo:IAO_0000115>A sinter terrace.</obo:IAO_0000115>
        <oboInOwl:hasOBONamespace>GAZ</oboInOwl:hasOBONamespace>
        <oboInOwl:id>GAZ:00146192</oboInOwl:id>
        <rdfs:label>Golden Fleece Terrace</rdfs:label>
    </owl:NamedIndividual>
    


    <!-- http://purl.obolibrary.org/obo/GAZ_00146193 -->

    <owl:NamedIndividual rdf:about="http://purl.obolibrary.org/obo/GAZ_00146193">
        <obo:RO_0001025 rdf:resource="http://purl.obolibrary.org/obo/GAZ_00146192"/>
        <obo:IAO_0000115>An active geyser.</obo:IAO_0000115>
        <oboInOwl:hasOBONamespace>GAZ</oboInOwl:hasOBONamespace>
        <oboInOwl:id>GAZ:00146193</oboInOwl:id>
        <rdfs:label>Wairiri Geyser</rdfs:label>
    </owl:NamedIndividual>
    


    <!-- http://purl.obolibrary.org/obo/GAZ_00146194 -->

    <owl:NamedIndividual rdf:about="http://purl.obolibrary.org/obo/GAZ_00146194">
        <obo:RO_0001025 rdf:resource="http://purl.obolibrary.org/obo/GAZ_00053854"/>
        <obo:IAO_0000115>A sinter terrace covered with clear blue alkali chloride pools and irregularly erupting geysers.</obo:IAO_0000115>
        <oboInOwl:hasOBONamespace>GAZ</oboInOwl:hasOBONamespace>
        <oboInOwl:id>GAZ:00146194</oboInOwl:id>
        <rdfs:label>Artist&apos;s Palette</rdfs:label>
    </owl:NamedIndividual>
    


    <!-- http://purl.obolibrary.org/obo/GAZ_00146195 -->

    <owl:NamedIndividual rdf:about="http://purl.obolibrary.org/obo/GAZ_00146195">
        <obo:RO_0001025 rdf:resource="http://purl.obolibrary.org/obo/GAZ_00053854"/>
        <obo:IAO_0000115>A cave extends 45 m, with a vertical drop of 23 m, to a shallow pool of clear, sulfate-rich, warm acid water.</obo:IAO_0000115>
        <oboInOwl:hasOBONamespace>GAZ</oboInOwl:hasOBONamespace>
        <oboInOwl:id>GAZ:00146195</oboInOwl:id>
        <rdfs:label>Ruatapu Cave</rdfs:label>
    </owl:NamedIndividual>
    


    <!-- http://purl.obolibrary.org/obo/GAZ_00146196 -->

    <owl:NamedIndividual rdf:about="http://purl.obolibrary.org/obo/GAZ_00146196">
        <obo:RO_0001025 rdf:resource="http://purl.obolibrary.org/obo/GAZ_00053854"/>
        <obo:IAO_0000115>A geyser.</obo:IAO_0000115>
        <oboInOwl:hasOBONamespace>GAZ</oboInOwl:hasOBONamespace>
        <oboInOwl:id>GAZ:00146196</oboInOwl:id>
        <rdfs:label>Soda Fountain</rdfs:label>
    </owl:NamedIndividual>
    


    <!-- http://purl.obolibrary.org/obo/GAZ_00146197 -->

    <owl:NamedIndividual rdf:about="http://purl.obolibrary.org/obo/GAZ_00146197">
        <obo:RO_0001025 rdf:resource="http://purl.obolibrary.org/obo/GAZ_00053854"/>
        <obo:IAO_0000115>An active geyser.</obo:IAO_0000115>
        <oboInOwl:hasOBONamespace>GAZ</oboInOwl:hasOBONamespace>
        <oboInOwl:id>GAZ:00146197</oboInOwl:id>
        <rdfs:label>Kurapai Geyser</rdfs:label>
    </owl:NamedIndividual>
    


    <!-- http://purl.obolibrary.org/obo/GAZ_00146198 -->

    <owl:NamedIndividual rdf:about="http://purl.obolibrary.org/obo/GAZ_00146198">
        <obo:RO_0001025 rdf:resource="http://purl.obolibrary.org/obo/GAZ_00053854"/>
        <obo:IAO_0000115>An active geyser.</obo:IAO_0000115>
        <oboInOwl:hasOBONamespace>GAZ</oboInOwl:hasOBONamespace>
        <oboInOwl:id>GAZ:00146198</oboInOwl:id>
        <rdfs:label>Ellan Vannin Geyser</rdfs:label>
    </owl:NamedIndividual>
    


    <!-- http://purl.obolibrary.org/obo/GAZ_00146199 -->

    <owl:NamedIndividual rdf:about="http://purl.obolibrary.org/obo/GAZ_00146199">
        <obo:RO_0001025 rdf:resource="http://purl.obolibrary.org/obo/GAZ_00053854"/>
        <obo:IAO_0000115>An active geyser.</obo:IAO_0000115>
        <oboInOwl:hasOBONamespace>GAZ</oboInOwl:hasOBONamespace>
        <oboInOwl:id>GAZ:00146199</oboInOwl:id>
        <rdfs:label>Benedix Washer Geyser</rdfs:label>
    </owl:NamedIndividual>
    


    <!-- http://purl.obolibrary.org/obo/GAZ_00146331 -->

    <owl:NamedIndividual rdf:about="http://purl.obolibrary.org/obo/GAZ_00146331">
        <obo:RO_0001025 rdf:resource="http://purl.obolibrary.org/obo/GAZ_00142875"/>
        <obo:IAO_0000115>A volcanic crater and now a lagoon in the Manukau Harbour, New Zealand, and is part of the Auckland volcanic field. Half-oval and about 600 m long, it has a small scoria island remaining in the centre with a horeshoe crater opening to the southwest.</obo:IAO_0000115>
        <oboInOwl:hasOBONamespace>GAZ</oboInOwl:hasOBONamespace>
        <oboInOwl:id>GAZ:00146331</oboInOwl:id>
        <rdfs:label>Mangere Lagoon</rdfs:label>
    </owl:NamedIndividual>
    


    <!-- http://purl.obolibrary.org/obo/GAZ_00146848 -->

    <owl:NamedIndividual rdf:about="http://purl.obolibrary.org/obo/GAZ_00146848">
        <obo:RO_0001025 rdf:resource="http://purl.obolibrary.org/obo/GAZ_00047005"/>
        <obo:IAO_0000115>A bay on the N of the Foveaux Strait.</obo:IAO_0000115>
        <oboInOwl:hasOBONamespace>GAZ</oboInOwl:hasOBONamespace>
        <oboInOwl:id>GAZ:00146848</oboInOwl:id>
        <rdfs:label>Colac Bay</rdfs:label>
    </owl:NamedIndividual>
    


    <!-- http://purl.obolibrary.org/obo/GAZ_00146849 -->

    <owl:NamedIndividual rdf:about="http://purl.obolibrary.org/obo/GAZ_00146849">
        <obo:RO_0001025 rdf:resource="http://purl.obolibrary.org/obo/GAZ_00142772"/>
        <obo:IAO_0000115>A former bay on the southern side of the Waitemata Harbour, formerly defining the original extent of the Auckland waterfront, Auckland, New Zealand. It was framed by two substantial headlands, Smale&apos;s Point dividing it from Freemans Bay in the west and Point Britomart dividing it from Official Bay and Mechanics Bay in the east. Now reclaimed.</obo:IAO_0000115>
        <oboInOwl:hasOBONamespace>GAZ</oboInOwl:hasOBONamespace>
        <oboInOwl:id>GAZ:00146849</oboInOwl:id>
        <rdfs:label>Commercial Bay</rdfs:label>
    </owl:NamedIndividual>
    


    <!-- http://purl.obolibrary.org/obo/GAZ_00146850 -->

    <owl:NamedIndividual rdf:about="http://purl.obolibrary.org/obo/GAZ_00146850">
        <obo:RO_0001025 rdf:resource="http://purl.obolibrary.org/obo/GAZ_00142772"/>
        <obo:IAO_0000115>A former bay in Waitemata Harbour in Auckland City, New Zealand. Now reclaimed.</obo:IAO_0000115>
        <oboInOwl:hasOBONamespace>GAZ</oboInOwl:hasOBONamespace>
        <oboInOwl:id>GAZ:00146850</oboInOwl:id>
        <rdfs:label>Mechanics Bay</rdfs:label>
    </owl:NamedIndividual>
    


    <!-- http://purl.obolibrary.org/obo/GAZ_00146851 -->

    <owl:NamedIndividual rdf:about="http://purl.obolibrary.org/obo/GAZ_00146851">
        <obo:RO_0001025 rdf:resource="http://purl.obolibrary.org/obo/GAZ_00046945"/>
        <obo:IAO_0000115>A wide bay on the Hauraki Gulf guarded by several islands, of which the largest is Whanganui Island.</obo:IAO_0000115>
        <oboInOwl:hasOBONamespace>GAZ</oboInOwl:hasOBONamespace>
        <oboInOwl:id>GAZ:00146851</oboInOwl:id>
        <rdfs:label>Coromandel Harbour</rdfs:label>
    </owl:NamedIndividual>
    


    <!-- http://purl.obolibrary.org/obo/GAZ_00146852 -->

    <owl:NamedIndividual rdf:about="http://purl.obolibrary.org/obo/GAZ_00146852">
        <obo:RO_0001025 rdf:resource="http://purl.obolibrary.org/obo/GAZ_00146864"/>
        <obo:IAO_0000115>A bay near the southern end of New Zealand&apos;s South Island.</obo:IAO_0000115>
        <oboInOwl:hasOBONamespace>GAZ</oboInOwl:hasOBONamespace>
        <oboInOwl:id>GAZ:00146852</oboInOwl:id>
        <rdfs:label>Curio Bay</rdfs:label>
    </owl:NamedIndividual>
    


    <!-- http://purl.obolibrary.org/obo/GAZ_00146853 -->

    <owl:NamedIndividual rdf:about="http://purl.obolibrary.org/obo/GAZ_00146853">
        <obo:RO_0001025 rdf:resource="http://purl.obolibrary.org/obo/GAZ_00142717"/>
        <obo:IAO_0000115>A bay located on the eastern side of Mount Stanley (971m) in Pelorus Sound, part of the Marlborough Sounds Maritime Park, located at the top of the South Island, New Zealand.</obo:IAO_0000115>
        <oboInOwl:hasOBONamespace>GAZ</oboInOwl:hasOBONamespace>
        <oboInOwl:id>GAZ:00146853</oboInOwl:id>
        <rdfs:label>Fairy Bay</rdfs:label>
    </owl:NamedIndividual>
    


    <!-- http://purl.obolibrary.org/obo/GAZ_00146854 -->

    <owl:NamedIndividual rdf:about="http://purl.obolibrary.org/obo/GAZ_00146854">
        <obo:RO_0001025 rdf:resource="http://purl.obolibrary.org/obo/GAZ_00004760"/>
        <obo:IAO_0000115>A former bay of Auckland, in the North Island of New Zealand. Now reclaimed.</obo:IAO_0000115>
        <oboInOwl:hasOBONamespace>GAZ</oboInOwl:hasOBONamespace>
        <oboInOwl:id>GAZ:00146854</oboInOwl:id>
        <rdfs:label>Freemans Bay</rdfs:label>
    </owl:NamedIndividual>
    


    <!-- http://purl.obolibrary.org/obo/GAZ_00146856 -->

    <owl:NamedIndividual rdf:about="http://purl.obolibrary.org/obo/GAZ_00146856">
        <obo:RO_0001025 rdf:resource="http://purl.obolibrary.org/obo/GAZ_00046945"/>
        <obo:IAO_0000115>A large bay which forms much of the north coast of Waiheke Island in northern New Zealand. The settlement of Onetangi lies in the centre of its coast.</obo:IAO_0000115>
        <oboInOwl:hasOBONamespace>GAZ</oboInOwl:hasOBONamespace>
        <oboInOwl:id>GAZ:00146856</oboInOwl:id>
        <rdfs:label>Onetangi Bay</rdfs:label>
    </owl:NamedIndividual>
    


    <!-- http://purl.obolibrary.org/obo/GAZ_00146857 -->

    <owl:NamedIndividual rdf:about="http://purl.obolibrary.org/obo/GAZ_00146857">
        <obo:RO_0001025 rdf:resource="http://purl.obolibrary.org/obo/GAZ_00046929"/>
        <obo:IAO_0000115>A bay located at the southern end of the North Island of New Zealand, to the southeast of Wellington. It runs for 40 km along the Cook Strait coast from Turakirae Head at the southern end of the Rimutaka Ranges to Cape Palliser, the North Island&apos;s southernmost point.</obo:IAO_0000115>
        <oboInOwl:hasOBONamespace>GAZ</oboInOwl:hasOBONamespace>
        <oboInOwl:id>GAZ:00146857</oboInOwl:id>
        <rdfs:label>Palliser Bay</rdfs:label>
    </owl:NamedIndividual>
    


    <!-- http://purl.obolibrary.org/obo/GAZ_00146858 -->

    <owl:NamedIndividual rdf:about="http://purl.obolibrary.org/obo/GAZ_00146858">
        <obo:RO_0001025 rdf:resource="http://purl.obolibrary.org/obo/GAZ_00142718"/>
        <obo:IAO_0000115>A bay located in Tennyson Inlet, within the Marlborough Sounds. Tennyson Inlet is an arm of Pelorus Sound.</obo:IAO_0000115>
        <oboInOwl:hasOBONamespace>GAZ</oboInOwl:hasOBONamespace>
        <oboInOwl:id>GAZ:00146858</oboInOwl:id>
        <rdfs:label>Penzance Bay</rdfs:label>
    </owl:NamedIndividual>
    


    <!-- http://purl.obolibrary.org/obo/GAZ_00146859 -->

    <owl:NamedIndividual rdf:about="http://purl.obolibrary.org/obo/GAZ_00146859">
        <obo:RO_0001025 rdf:resource="http://purl.obolibrary.org/obo/GAZ_00142718"/>
        <obo:IAO_0000115>A bay to the S of Penzance Bay.</obo:IAO_0000115>
        <oboInOwl:hasOBONamespace>GAZ</oboInOwl:hasOBONamespace>
        <oboInOwl:id>GAZ:00146859</oboInOwl:id>
        <rdfs:label>Tuna Bay</rdfs:label>
    </owl:NamedIndividual>
    


    <!-- http://purl.obolibrary.org/obo/GAZ_00146860 -->

    <owl:NamedIndividual rdf:about="http://purl.obolibrary.org/obo/GAZ_00146860">
        <obo:RO_0001025 rdf:resource="http://purl.obolibrary.org/obo/GAZ_00142718"/>
        <obo:IAO_0000115>A bay.</obo:IAO_0000115>
        <oboInOwl:hasOBONamespace>GAZ</oboInOwl:hasOBONamespace>
        <oboInOwl:id>GAZ:00146860</oboInOwl:id>
        <rdfs:label>Duncan Bay</rdfs:label>
    </owl:NamedIndividual>
    


    <!-- http://purl.obolibrary.org/obo/GAZ_00146861 -->

    <owl:NamedIndividual rdf:about="http://purl.obolibrary.org/obo/GAZ_00146861">
        <obo:RO_0001025 rdf:resource="http://purl.obolibrary.org/obo/GAZ_00142718"/>
        <obo:IAO_0000115>A bay.</obo:IAO_0000115>
        <oboInOwl:hasOBONamespace>GAZ</oboInOwl:hasOBONamespace>
        <oboInOwl:id>GAZ:00146861</oboInOwl:id>
        <rdfs:label>Elaine Bay</rdfs:label>
    </owl:NamedIndividual>
    


    <!-- http://purl.obolibrary.org/obo/GAZ_00146862 -->

    <owl:NamedIndividual rdf:about="http://purl.obolibrary.org/obo/GAZ_00146862">
        <obo:RO_0001025 rdf:resource="http://purl.obolibrary.org/obo/GAZ_00007126"/>
        <obo:IAO_0000115>A large bay which comprises about half of the west coast of Chatham Island/Rekohu.</obo:IAO_0000115>
        <oboInOwl:hasOBONamespace>GAZ</oboInOwl:hasOBONamespace>
        <oboInOwl:id>GAZ:00146862</oboInOwl:id>
        <rdfs:label>Petre Bay</rdfs:label>
    </owl:NamedIndividual>
    


    <!-- http://purl.obolibrary.org/obo/GAZ_00146863 -->

    <owl:NamedIndividual rdf:about="http://purl.obolibrary.org/obo/GAZ_00146863">
        <obo:RO_0001025 rdf:resource="http://purl.obolibrary.org/obo/GAZ_00146862"/>
        <obo:IAO_0000115>A bay within Petre Bay.</obo:IAO_0000115>
        <oboInOwl:hasOBONamespace>GAZ</oboInOwl:hasOBONamespace>
        <oboInOwl:id>GAZ:00146863</oboInOwl:id>
        <rdfs:label>Waitangi Bay</rdfs:label>
    </owl:NamedIndividual>
    


    <!-- http://purl.obolibrary.org/obo/GAZ_00146864 -->

    <owl:NamedIndividual rdf:about="http://purl.obolibrary.org/obo/GAZ_00146864">
        <obo:RO_0001025 rdf:resource="http://purl.obolibrary.org/obo/GAZ_00004767"/>
        <obo:RO_0001025 rdf:resource="http://purl.obolibrary.org/obo/GAZ_00008572"/>
        <obo:IAO_0000115>An area in the southeastern corner of the South Island of New Zealand. The area lies between Balclutha and Invercargill, straddling the boundary between the Otago and Southland regions. It includes the South Island&apos;s southernmost point, Slope Point.</obo:IAO_0000115>
        <oboInOwl:hasOBONamespace>GAZ</oboInOwl:hasOBONamespace>
        <oboInOwl:id>GAZ:00146864</oboInOwl:id>
        <rdfs:label>The Catlins</rdfs:label>
    </owl:NamedIndividual>
    


    <!-- http://purl.obolibrary.org/obo/GAZ_00146865 -->

    <owl:NamedIndividual rdf:about="http://purl.obolibrary.org/obo/GAZ_00146865">
        <obo:RO_0001025 rdf:resource="http://purl.obolibrary.org/obo/GAZ_00146864"/>
        <obo:IAO_0000115>A bay located in the Catlins on the southern coast of New Zealand&apos;s South Island. The bay sweeps gently from North Head, at the entrance to Waikawa Harbour, around to South Head.</obo:IAO_0000115>
        <oboInOwl:hasOBONamespace>GAZ</oboInOwl:hasOBONamespace>
        <oboInOwl:id>GAZ:00146865</oboInOwl:id>
        <rdfs:label>Porpoise Bay</rdfs:label>
    </owl:NamedIndividual>
    


    <!-- http://purl.obolibrary.org/obo/GAZ_00146866 -->

    <owl:NamedIndividual rdf:about="http://purl.obolibrary.org/obo/GAZ_00146866">
        <obo:RO_0001025 rdf:resource="http://purl.obolibrary.org/obo/GAZ_00146864"/>
        <obo:IAO_0000115>The southernmost point of the South Island of New Zealand.</obo:IAO_0000115>
        <oboInOwl:hasOBONamespace>GAZ</oboInOwl:hasOBONamespace>
        <oboInOwl:id>GAZ:00146866</oboInOwl:id>
        <rdfs:label>Slope Point</rdfs:label>
    </owl:NamedIndividual>
    


    <!-- http://purl.obolibrary.org/obo/GAZ_00146867 -->

    <owl:NamedIndividual rdf:about="http://purl.obolibrary.org/obo/GAZ_00146867">
        <obo:RO_0001025 rdf:resource="http://purl.obolibrary.org/obo/GAZ_00142731"/>
        <obo:IAO_0000115>A sheltered harbour which forms the north-east extension of Cloudy Bay at the northeast of New Zealand&apos;s South Island, on the east coast of the Marlborough Sounds.</obo:IAO_0000115>
        <oboInOwl:hasOBONamespace>GAZ</oboInOwl:hasOBONamespace>
        <oboInOwl:id>GAZ:00146867</oboInOwl:id>
        <rdfs:label>Port Underwood</rdfs:label>
    </owl:NamedIndividual>
    


    <!-- http://purl.obolibrary.org/obo/GAZ_00146868 -->

    <owl:NamedIndividual rdf:about="http://purl.obolibrary.org/obo/GAZ_00146868">
        <obo:RO_0001025 rdf:resource="http://purl.obolibrary.org/obo/GAZ_00046929"/>
        <obo:IAO_0000115>A bay located between Houghton Bay and Te Raekaihau Point, on the rocky shores of the Cook Strait.</obo:IAO_0000115>
        <oboInOwl:hasOBONamespace>GAZ</oboInOwl:hasOBONamespace>
        <oboInOwl:id>GAZ:00146868</oboInOwl:id>
        <rdfs:label>Princess Bay</rdfs:label>
    </owl:NamedIndividual>
    


    <!-- http://purl.obolibrary.org/obo/GAZ_00146869 -->

    <owl:NamedIndividual rdf:about="http://purl.obolibrary.org/obo/GAZ_00146869">
        <obo:RO_0001025 rdf:resource="http://purl.obolibrary.org/obo/GAZ_00004767"/>
        <obo:IAO_0000115>A long, rugged indented finger of land that forms the easternmost part of Dunedin, New Zealand. Volcanic in origin, it forms one wall of the collapsed crater that now forms Otago Harbour. The peninsula lies due east of Otago Harbour and runs parallel to the mainland for 30 km. Its maximum width is 12 km. It is joined to the mainland at the south-west end by a narrow isthmus a little over1 km in width.</obo:IAO_0000115>
        <oboInOwl:hasOBONamespace>GAZ</oboInOwl:hasOBONamespace>
        <oboInOwl:id>GAZ:00146869</oboInOwl:id>
        <rdfs:label>Otago Peninsula</rdfs:label>
    </owl:NamedIndividual>
    


    <!-- http://purl.obolibrary.org/obo/GAZ_00146870 -->

    <owl:NamedIndividual rdf:about="http://purl.obolibrary.org/obo/GAZ_00146870">
        <rdf:type rdf:resource="http://purl.obolibrary.org/obo/ENVO_00000305"/>
        <obo:RO_0001025 rdf:resource="http://purl.obolibrary.org/obo/GAZ_00004768"/>
        <obo:RO_0001025 rdf:resource="http://purl.obolibrary.org/obo/GAZ_00146869"/>
        <obo:IAO_0000115>A headland at the end of the Otago Peninsula in New Zealand, overlooking the mouth of the Otago Harbour. It lies within the city limits of Dunedin.</obo:IAO_0000115>
        <oboInOwl:hasOBONamespace>GAZ</oboInOwl:hasOBONamespace>
        <oboInOwl:id>GAZ:00146870</oboInOwl:id>
        <rdfs:label>Taiaroa Head</rdfs:label>
    </owl:NamedIndividual>
    


    <!-- http://purl.obolibrary.org/obo/GAZ_00146871 -->

    <owl:NamedIndividual rdf:about="http://purl.obolibrary.org/obo/GAZ_00146871">
        <obo:RO_0001025 rdf:resource="http://purl.obolibrary.org/obo/GAZ_00146869"/>
        <obo:IAO_0000115>A tidal inlet on the Pacific coast of the Otago Peninsula.</obo:IAO_0000115>
        <oboInOwl:hasOBONamespace>GAZ</oboInOwl:hasOBONamespace>
        <oboInOwl:id>GAZ:00146871</oboInOwl:id>
        <rdfs:label>Hoopers Inlet</rdfs:label>
    </owl:NamedIndividual>
    


    <!-- http://purl.obolibrary.org/obo/GAZ_00146872 -->

    <owl:NamedIndividual rdf:about="http://purl.obolibrary.org/obo/GAZ_00146872">
        <obo:RO_0001025 rdf:resource="http://purl.obolibrary.org/obo/GAZ_00146869"/>
        <obo:IAO_0000115>A tidal inlet on the Pacific coast of the Otago Peninsula.</obo:IAO_0000115>
        <oboInOwl:hasOBONamespace>GAZ</oboInOwl:hasOBONamespace>
        <oboInOwl:id>GAZ:00146872</oboInOwl:id>
        <rdfs:label>Papanui Inlet</rdfs:label>
    </owl:NamedIndividual>
    


    <!-- http://purl.obolibrary.org/obo/GAZ_00146873 -->

    <owl:NamedIndividual rdf:about="http://purl.obolibrary.org/obo/GAZ_00146873">
        <rdf:type rdf:resource="http://purl.obolibrary.org/obo/ENVO_00000305"/>
        <obo:RO_0001025 rdf:resource="http://purl.obolibrary.org/obo/GAZ_00146869"/>
        <obo:IAO_0000115>A headland on the Pacific coast of the Otago Peninsula, betwen Hoopers Inlet and Papanui Inlet.</obo:IAO_0000115>
        <oboInOwl:hasOBONamespace>GAZ</oboInOwl:hasOBONamespace>
        <oboInOwl:id>GAZ:00146873</oboInOwl:id>
        <rdfs:label>Cape Saunders</rdfs:label>
    </owl:NamedIndividual>
    


    <!-- http://purl.obolibrary.org/obo/GAZ_00146874 -->

    <owl:NamedIndividual rdf:about="http://purl.obolibrary.org/obo/GAZ_00146874">
        <obo:RO_0001025 rdf:resource="http://purl.obolibrary.org/obo/GAZ_00146869"/>
        <obo:IAO_0000115>A sandy bay with large dunes, located on the eastern side of the Otago Peninsula, New Zealand, 15km east of central Dunedin.</obo:IAO_0000115>
        <oboInOwl:hasOBONamespace>GAZ</oboInOwl:hasOBONamespace>
        <oboInOwl:id>GAZ:00146874</oboInOwl:id>
        <rdfs:label>Sandfly Bay</rdfs:label>
    </owl:NamedIndividual>
    


    <!-- http://purl.obolibrary.org/obo/GAZ_00146876 -->

    <owl:NamedIndividual rdf:about="http://purl.obolibrary.org/obo/GAZ_00146876">
        <obo:RO_0001025 rdf:resource="http://purl.obolibrary.org/obo/GAZ_00030189"/>
        <obo:IAO_0000115>A bay in Abel Tasman National Park.</obo:IAO_0000115>
        <oboInOwl:hasOBONamespace>GAZ</oboInOwl:hasOBONamespace>
        <oboInOwl:id>GAZ:00146876</oboInOwl:id>
        <rdfs:label>Torrent Bay</rdfs:label>
    </owl:NamedIndividual>
    


    <!-- http://purl.obolibrary.org/obo/GAZ_00146877 -->

    <owl:NamedIndividual rdf:about="http://purl.obolibrary.org/obo/GAZ_00146877">
        <obo:RO_0001025 rdf:resource="http://purl.obolibrary.org/obo/GAZ_00046929"/>
        <obo:RO_0001025 rdf:resource="http://purl.obolibrary.org/obo/GAZ_00146878"/>
        <obo:IAO_0000115>A bay Wellington, New Zealand is located along the beach from Seatoun and over the hill from Miramar on the Miramar Peninsula.</obo:IAO_0000115>
        <oboInOwl:hasOBONamespace>GAZ</oboInOwl:hasOBONamespace>
        <oboInOwl:id>GAZ:00146877</oboInOwl:id>
        <rdfs:label>Worser Bay</rdfs:label>
    </owl:NamedIndividual>
    


    <!-- http://purl.obolibrary.org/obo/GAZ_00146878 -->

    <owl:NamedIndividual rdf:about="http://purl.obolibrary.org/obo/GAZ_00146878">
        <obo:RO_0001025 rdf:resource="http://purl.obolibrary.org/obo/GAZ_00008565"/>
        <obo:RO_0001025 rdf:resource="http://purl.obolibrary.org/obo/GAZ_00009760"/>
        <obo:IAO_0000115>A peninsula at the southeastern end of the city of Wellington, New Zealand. It contains the suburbs of Miramar, Maupuia, Strathmore and Seatoun. The isthmus connecting the peninsula to the rest of Wellington separates Evans Bay to the north from Lyall Bay to the south.</obo:IAO_0000115>
        <oboInOwl:hasOBONamespace>GAZ</oboInOwl:hasOBONamespace>
        <oboInOwl:id>GAZ:00146878</oboInOwl:id>
        <rdfs:label>Miramar Peninsula</rdfs:label>
    </owl:NamedIndividual>
    


    <!-- http://purl.obolibrary.org/obo/GAZ_00146879 -->

    <owl:NamedIndividual rdf:about="http://purl.obolibrary.org/obo/GAZ_00146879">
        <obo:RO_0001025 rdf:resource="http://purl.obolibrary.org/obo/GAZ_00046929"/>
        <obo:RO_0001025 rdf:resource="http://purl.obolibrary.org/obo/GAZ_00146878"/>
        <obo:IAO_0000115>A bay.</obo:IAO_0000115>
        <oboInOwl:hasOBONamespace>GAZ</oboInOwl:hasOBONamespace>
        <oboInOwl:id>GAZ:00146879</oboInOwl:id>
        <rdfs:label>Evans Bay</rdfs:label>
    </owl:NamedIndividual>
    


    <!-- http://purl.obolibrary.org/obo/GAZ_00146880 -->

    <owl:NamedIndividual rdf:about="http://purl.obolibrary.org/obo/GAZ_00146880">
        <obo:RO_0001025 rdf:resource="http://purl.obolibrary.org/obo/GAZ_00046976"/>
        <obo:IAO_0000115>A cluster of rocks that lies on the western side of the entrance of Wellington Harbour, on the approaches to the city of Wellington.</obo:IAO_0000115>
        <oboInOwl:hasOBONamespace>GAZ</oboInOwl:hasOBONamespace>
        <oboInOwl:id>GAZ:00146880</oboInOwl:id>
        <rdfs:label>Barrett Reef</rdfs:label>
    </owl:NamedIndividual>
    


    <!-- http://purl.obolibrary.org/obo/GAZ_00147128 -->

    <owl:NamedIndividual rdf:about="http://purl.obolibrary.org/obo/GAZ_00147128">
        <rdf:type rdf:resource="http://purl.obolibrary.org/obo/ENVO_00000305"/>
        <obo:RO_0001025 rdf:resource="http://purl.obolibrary.org/obo/GAZ_00004778"/>
        <obo:IAO_0000115>A headland on the West Coast of New Zealand&apos;s South Island. It is located north of the village of Whataroa and west of Harihari, and is southwest of the Westland District&apos;s main centre, Hokitika. On the southern side of the headland, the Whataroa River meets the Tasman Sea. To the east is the Saltwater Lagoon.</obo:IAO_0000115>
        <oboInOwl:hasOBONamespace>GAZ</oboInOwl:hasOBONamespace>
        <oboInOwl:id>GAZ:00147128</oboInOwl:id>
        <rdfs:label>Abut Head</rdfs:label>
    </owl:NamedIndividual>
    


    <!-- http://purl.obolibrary.org/obo/GAZ_00147129 -->

    <owl:NamedIndividual rdf:about="http://purl.obolibrary.org/obo/GAZ_00147129">
        <obo:RO_0001025 rdf:resource="http://purl.obolibrary.org/obo/GAZ_00004760"/>
        <obo:IAO_0000115>A rocky point on the headland at the eastern end of the small sandy beach named Ladies Bay, Auckland, New Zealand.</obo:IAO_0000115>
        <oboInOwl:hasOBONamespace>GAZ</oboInOwl:hasOBONamespace>
        <oboInOwl:id>GAZ:00147129</oboInOwl:id>
        <rdfs:label>Achilles Point</rdfs:label>
    </owl:NamedIndividual>
    


    <!-- http://purl.obolibrary.org/obo/GAZ_00147130 -->

    <owl:NamedIndividual rdf:about="http://purl.obolibrary.org/obo/GAZ_00147130">
        <obo:RO_0001025 rdf:resource="http://purl.obolibrary.org/obo/GAZ_00004777"/>
        <obo:RO_0001025 rdf:resource="http://purl.obolibrary.org/obo/GAZ_00058654"/>
        <obo:IAO_0000115>A located on the southwestern coast of New Zealand&apos;s South Island, 40 kmmetres north of Milford Sound, and 15 km north of the mouth of the Hollyford River. Traditionally, Awarua Point is regarded as the end of Fiordland and the start of the West Coast region, although the boundary of Fiordland National Park is located 10 km further south at the northern end of Martins Bay.</obo:IAO_0000115>
        <oboInOwl:hasOBONamespace>GAZ</oboInOwl:hasOBONamespace>
        <oboInOwl:id>GAZ:00147130</oboInOwl:id>
        <rdfs:label>Awarua Point</rdfs:label>
    </owl:NamedIndividual>
    


    <!-- http://purl.obolibrary.org/obo/GAZ_00147131 -->

    <owl:NamedIndividual rdf:about="http://purl.obolibrary.org/obo/GAZ_00147131">
        <obo:RO_0001025 rdf:resource="http://purl.obolibrary.org/obo/GAZ_00029928"/>
        <oboInOwl:hasOBONamespace>GAZ</oboInOwl:hasOBONamespace>
        <oboInOwl:id>GAZ:00147131</oboInOwl:id>
        <rdfs:label>Cape Brett Peninsula</rdfs:label>
    </owl:NamedIndividual>
    


    <!-- http://purl.obolibrary.org/obo/GAZ_00147132 -->

    <owl:NamedIndividual rdf:about="http://purl.obolibrary.org/obo/GAZ_00147132">
        <rdf:type rdf:resource="http://purl.obolibrary.org/obo/ENVO_00000305"/>
        <obo:RO_0001025 rdf:resource="http://purl.obolibrary.org/obo/GAZ_00147131"/>
        <obo:IAO_0000115>A headland on the northern North Island coast in New Zealand. Located at the end of the 15 km long Cape Brett Peninsula, the head extends north into the Pacific Ocean at the eastern end of the Bay of Islands.</obo:IAO_0000115>
        <oboInOwl:hasOBONamespace>GAZ</oboInOwl:hasOBONamespace>
        <oboInOwl:id>GAZ:00147132</oboInOwl:id>
        <rdfs:label>Cape Brett</rdfs:label>
    </owl:NamedIndividual>
    


    <!-- http://purl.obolibrary.org/obo/GAZ_00147134 -->

    <owl:NamedIndividual rdf:about="http://purl.obolibrary.org/obo/GAZ_00147134">
        <rdf:type rdf:resource="http://purl.obolibrary.org/obo/ENVO_00000305"/>
        <obo:RO_0001025 rdf:resource="http://purl.obolibrary.org/obo/GAZ_00004760"/>
        <obo:IAO_0000115>A former headland in the Waitemata Harbour, Auckland, New Zealand. Located between Commercial Bay and Official Bay, it was later quarried away to produce fill for land reclamation in Mechanics Bay.</obo:IAO_0000115>
        <oboInOwl:hasOBONamespace>GAZ</oboInOwl:hasOBONamespace>
        <oboInOwl:id>GAZ:00147134</oboInOwl:id>
        <rdfs:label>Point Britomart</rdfs:label>
    </owl:NamedIndividual>
    


    <!-- http://purl.obolibrary.org/obo/GAZ_00147135 -->

    <owl:NamedIndividual rdf:about="http://purl.obolibrary.org/obo/GAZ_00147135">
        <rdf:type rdf:resource="http://purl.obolibrary.org/obo/ENVO_00000305"/>
        <obo:RO_0001025 rdf:resource="http://purl.obolibrary.org/obo/GAZ_00008568"/>
        <obo:IAO_0000115>A cape located in Marlborough, New Zealand, on the northeastern coast of the South Island. It lies at the southern end of Clifford Bay, 15 km northeast of Ward, and 42 km southeast of Blenheim.</obo:IAO_0000115>
        <oboInOwl:hasOBONamespace>GAZ</oboInOwl:hasOBONamespace>
        <oboInOwl:id>GAZ:00147135</oboInOwl:id>
        <rdfs:label>Cape Campbell</rdfs:label>
    </owl:NamedIndividual>
    


    <!-- http://purl.obolibrary.org/obo/GAZ_00147136 -->

    <owl:NamedIndividual rdf:about="http://purl.obolibrary.org/obo/GAZ_00147136">
        <obo:RO_0001025 rdf:resource="http://purl.obolibrary.org/obo/GAZ_00008568"/>
        <obo:IAO_0000115>A shallow lagoon protected from the open sea by a single barrier beach covered by sand dunes. It is on the north-easterly extension of the Ward depression.</obo:IAO_0000115>
        <oboInOwl:hasOBONamespace>GAZ</oboInOwl:hasOBONamespace>
        <oboInOwl:id>GAZ:00147136</oboInOwl:id>
        <rdfs:label>Lake Grassmere</rdfs:label>
    </owl:NamedIndividual>
    


    <!-- http://purl.obolibrary.org/obo/GAZ_00147137 -->

    <owl:NamedIndividual rdf:about="http://purl.obolibrary.org/obo/GAZ_00147137">
        <obo:RO_0001025 rdf:resource="http://purl.obolibrary.org/obo/GAZ_00030217"/>
        <obo:IAO_0000115>Two parallel ranges of mountains in the northeast of the South Island of New Zealand. Formed along New Zealand&apos;s Alpine Fault, they can be seen as the northernmost extension of the Southern Alps in the South Island. The long straight river valley of the Clarence River separate the Seaward Kaikouras from the longer and loftier Inland Kaikouras.</obo:IAO_0000115>
        <oboInOwl:hasOBONamespace>GAZ</oboInOwl:hasOBONamespace>
        <oboInOwl:id>GAZ:00147137</oboInOwl:id>
        <rdfs:label>Kaikoura Ranges</rdfs:label>
    </owl:NamedIndividual>
    


    <!-- http://purl.obolibrary.org/obo/GAZ_00147138 -->

    <owl:NamedIndividual rdf:about="http://purl.obolibrary.org/obo/GAZ_00147138">
        <obo:RO_0001025 rdf:resource="http://purl.obolibrary.org/obo/GAZ_00147137"/>
        <obo:IAO_0000115>One of the Kaikouras Ranges.</obo:IAO_0000115>
        <oboInOwl:hasOBONamespace>GAZ</oboInOwl:hasOBONamespace>
        <oboInOwl:id>GAZ:00147138</oboInOwl:id>
        <rdfs:label>Inland Kaikouras</rdfs:label>
    </owl:NamedIndividual>
    


    <!-- http://purl.obolibrary.org/obo/GAZ_00147139 -->

    <owl:NamedIndividual rdf:about="http://purl.obolibrary.org/obo/GAZ_00147139">
        <obo:RO_0001025 rdf:resource="http://purl.obolibrary.org/obo/GAZ_00147137"/>
        <obo:IAO_0000115>One of the Kaikouras Ranges.</obo:IAO_0000115>
        <oboInOwl:hasOBONamespace>GAZ</oboInOwl:hasOBONamespace>
        <oboInOwl:id>GAZ:00147139</oboInOwl:id>
        <rdfs:label>Seaward Kaikouras</rdfs:label>
    </owl:NamedIndividual>
    


    <!-- http://purl.obolibrary.org/obo/GAZ_00147140 -->

    <owl:NamedIndividual rdf:about="http://purl.obolibrary.org/obo/GAZ_00147140">
        <obo:RO_0001025 rdf:resource="http://purl.obolibrary.org/obo/GAZ_00146174"/>
        <obo:IAO_0000115>The northernmost point of the Coromandel Peninsula in New Zealand&apos;s North Island. It lies 85 km north of Thames, and 70 km northeast of the city of Auckland, on the other side of the Hauraki Gulf.</obo:IAO_0000115>
        <oboInOwl:hasOBONamespace>GAZ</oboInOwl:hasOBONamespace>
        <oboInOwl:id>GAZ:00147140</oboInOwl:id>
        <rdfs:label>Cape Colville</rdfs:label>
    </owl:NamedIndividual>
    


    <!-- http://purl.obolibrary.org/obo/GAZ_00147141 -->

    <owl:NamedIndividual rdf:about="http://purl.obolibrary.org/obo/GAZ_00147141">
        <obo:RO_0001025 rdf:resource="http://purl.obolibrary.org/obo/GAZ_00010248"/>
        <obo:IAO_0000115>The easternmost point of the main islands of New Zealand. It is located to the north of Gisborne in the northeast of the North Island.</obo:IAO_0000115>
        <oboInOwl:hasOBONamespace>GAZ</oboInOwl:hasOBONamespace>
        <oboInOwl:id>GAZ:00147141</oboInOwl:id>
        <rdfs:label>East Cape</rdfs:label>
    </owl:NamedIndividual>
    


    <!-- http://purl.obolibrary.org/obo/GAZ_00147142 -->

    <owl:NamedIndividual rdf:about="http://purl.obolibrary.org/obo/GAZ_00147142">
        <obo:RO_0001025 rdf:resource="http://purl.obolibrary.org/obo/GAZ_00010256"/>
        <obo:IAO_0000115>Mountains is located in inland Hawke&apos;s Bay in the eastern North Island of New Zealand. The range lies between the city of Napier, 55 km to the southeast, and Lake Taupo, 50 km to the northwest. It is the source of many rivers which flow into Hawke Bay, including among them the Tutaekuri, Mohaka, and Ngaruroro Rivers.</obo:IAO_0000115>
        <oboInOwl:hasOBONamespace>GAZ</oboInOwl:hasOBONamespace>
        <oboInOwl:id>GAZ:00147142</oboInOwl:id>
        <rdfs:label>Kaweka Range</rdfs:label>
    </owl:NamedIndividual>
    


    <!-- http://purl.obolibrary.org/obo/GAZ_00147143 -->

    <owl:NamedIndividual rdf:about="http://purl.obolibrary.org/obo/GAZ_00147143">
        <obo:RO_0001025 rdf:resource="http://purl.obolibrary.org/obo/GAZ_00010256"/>
        <obo:IAO_0000115>A mountain range that runs northeast-southwest for 110 km from inland Hawke&apos;s Bay to near Woodville. It is separated in the south from the northern end of the Tararua Range by the Manawatu Gorge.</obo:IAO_0000115>
        <oboInOwl:hasOBONamespace>GAZ</oboInOwl:hasOBONamespace>
        <oboInOwl:id>GAZ:00147143</oboInOwl:id>
        <rdfs:label>Ruahine Range</rdfs:label>
    </owl:NamedIndividual>
    


    <!-- http://purl.obolibrary.org/obo/GAZ_00147144 -->

    <owl:NamedIndividual rdf:about="http://purl.obolibrary.org/obo/GAZ_00147144">
        <obo:RO_0001025 rdf:resource="http://purl.obolibrary.org/obo/GAZ_00004765"/>
        <obo:IAO_0000115>A mountain range that runs southwest-northeast for 55 km from Turakirae Head at the eastern end of Palliser Bay to the upper reaches of the Hutt Valley where it joins the southern end of the Tararua Range.</obo:IAO_0000115>
        <oboInOwl:hasOBONamespace>GAZ</oboInOwl:hasOBONamespace>
        <oboInOwl:id>GAZ:00147144</oboInOwl:id>
        <rdfs:label>Rimutaka Range</rdfs:label>
    </owl:NamedIndividual>
    


    <!-- http://purl.obolibrary.org/obo/GAZ_00147145 -->

    <owl:NamedIndividual rdf:about="http://purl.obolibrary.org/obo/GAZ_00147145">
        <rdf:type rdf:resource="http://purl.obolibrary.org/obo/ENVO_00000100"/>
        <obo:RO_0001025 rdf:resource="http://purl.obolibrary.org/obo/GAZ_00004772"/>
        <obo:RO_0001025 rdf:resource="http://purl.obolibrary.org/obo/GAZ_00010256"/>
        <obo:IAO_0000115>A gorge that runs between the Ruahine and Tararua Ranges of the North Island of New Zealand, linking the Manawatu and Hawke&apos;s Bay regions. It lies to the northeast of Palmerston North - its western end is near the small town of Ashhurst, its eastern end is close to the town of Woodville.</obo:IAO_0000115>
        <oboInOwl:hasOBONamespace>GAZ</oboInOwl:hasOBONamespace>
        <oboInOwl:id>GAZ:00147145</oboInOwl:id>
        <rdfs:label>Manawatu Gorge</rdfs:label>
    </owl:NamedIndividual>
    


    <!-- http://purl.obolibrary.org/obo/GAZ_00147146 -->

    <owl:NamedIndividual rdf:about="http://purl.obolibrary.org/obo/GAZ_00147146">
        <obo:RO_0001025 rdf:resource="http://purl.obolibrary.org/obo/GAZ_00004765"/>
        <obo:IAO_0000115>A mountain range that lies north of Gisborne, near East Cape in New Zealand&apos;s North Island. It forms part of the North Island&apos;s main mountain chain, which runs north-northeast from Wellington to East Cape.</obo:IAO_0000115>
        <oboInOwl:hasOBONamespace>GAZ</oboInOwl:hasOBONamespace>
        <oboInOwl:id>GAZ:00147146</oboInOwl:id>
        <rdfs:label>Raukumara Range</rdfs:label>
    </owl:NamedIndividual>
    


    <!-- http://purl.obolibrary.org/obo/GAZ_00147147 -->

    <owl:NamedIndividual rdf:about="http://purl.obolibrary.org/obo/GAZ_00147147">
        <obo:RO_0001025 rdf:resource="http://purl.obolibrary.org/obo/GAZ_00004765"/>
        <obo:IAO_0000115>A peninsula located on the east coast of New Zealand&apos;s North Island, between the cities of Napier and Gisborne. The peninsula is 21.7 km long and 11.3 km wide rising to its highest point at Rahuimokairoa reaching about 403 m above sea level. Mahia was initially an island which over time, has had a sand bar join it to the North Island.</obo:IAO_0000115>
        <oboInOwl:hasOBONamespace>GAZ</oboInOwl:hasOBONamespace>
        <oboInOwl:id>GAZ:00147147</oboInOwl:id>
        <rdfs:label>Mahia Peninsula</rdfs:label>
    </owl:NamedIndividual>
    


    <!-- http://purl.obolibrary.org/obo/GAZ_00147148 -->

    <owl:NamedIndividual rdf:about="http://purl.obolibrary.org/obo/GAZ_00147148">
        <obo:RO_0001025 rdf:resource="http://purl.obolibrary.org/obo/GAZ_00008564"/>
        <obo:IAO_0000115>The westernmost point of Taranaki, on the west coast of New Zealand&apos;s North Island. It is located close to the volcanic cone of Mount Taranaki.</obo:IAO_0000115>
        <oboInOwl:hasOBONamespace>GAZ</oboInOwl:hasOBONamespace>
        <oboInOwl:id>GAZ:00147148</oboInOwl:id>
        <rdfs:label>Cape Egmont</rdfs:label>
    </owl:NamedIndividual>
    


    <!-- http://purl.obolibrary.org/obo/GAZ_00147149 -->

    <owl:NamedIndividual rdf:about="http://purl.obolibrary.org/obo/GAZ_00147149">
        <rdf:type rdf:resource="http://purl.obolibrary.org/obo/ENVO_00000305"/>
        <obo:RO_0001025 rdf:resource="http://purl.obolibrary.org/obo/GAZ_00008563"/>
        <obo:IAO_0000115>A headland in New Zealand, the most northerly point on the South Island. It is located just west of Farewell Spit.</obo:IAO_0000115>
        <oboInOwl:hasOBONamespace>GAZ</oboInOwl:hasOBONamespace>
        <oboInOwl:id>GAZ:00147149</oboInOwl:id>
        <rdfs:label>Cape Farewell</rdfs:label>
    </owl:NamedIndividual>
    


    <!-- http://purl.obolibrary.org/obo/GAZ_00147150 -->

    <owl:NamedIndividual rdf:about="http://purl.obolibrary.org/obo/GAZ_00147150">
        <obo:RO_0001025 rdf:resource="http://purl.obolibrary.org/obo/GAZ_00008563"/>
        <obo:IAO_0000115>A narrow sand spit situated at the northern end of the South Island of New Zealand. It runs eastwards from Cape Farewell, the island&apos;s northernmost point. It is located about 50 km north of Takaka and 20 km from Collingwood. It forms the northern side of Golden Bay.</obo:IAO_0000115>
        <oboInOwl:hasOBONamespace>GAZ</oboInOwl:hasOBONamespace>
        <oboInOwl:id>GAZ:00147150</oboInOwl:id>
        <rdfs:label>Farewell Spit</rdfs:label>
    </owl:NamedIndividual>
    


    <!-- http://purl.obolibrary.org/obo/GAZ_00147151 -->

    <owl:NamedIndividual rdf:about="http://purl.obolibrary.org/obo/GAZ_00147151">
        <obo:RO_0001025 rdf:resource="http://purl.obolibrary.org/obo/GAZ_00004764"/>
        <obo:IAO_0000115>A mountain range in the central north of New Zealand&apos;s South Island. It lies between Lake Rotoiti and the upper reaches of the Wairau River, and marks the eastern boundary of Nelson Lakes National Park.</obo:IAO_0000115>
        <oboInOwl:hasOBONamespace>GAZ</oboInOwl:hasOBONamespace>
        <oboInOwl:id>GAZ:00147151</oboInOwl:id>
        <rdfs:label>Saint Arnaud Range</rdfs:label>
    </owl:NamedIndividual>
    


    <!-- http://purl.obolibrary.org/obo/GAZ_00147152 -->

    <owl:NamedIndividual rdf:about="http://purl.obolibrary.org/obo/GAZ_00147152">
        <obo:RO_0001025 rdf:resource="http://purl.obolibrary.org/obo/GAZ_00029959"/>
        <obo:IAO_0000115>A prominent headland on the West Coast of New Zealand&apos;s South Island, overlooking the Tasman Sea. It is located ten km west of the town of Westport.</obo:IAO_0000115>
        <oboInOwl:hasOBONamespace>GAZ</oboInOwl:hasOBONamespace>
        <oboInOwl:id>GAZ:00147152</oboInOwl:id>
        <rdfs:label>Cape Foulwind</rdfs:label>
    </owl:NamedIndividual>
    


    <!-- http://purl.obolibrary.org/obo/GAZ_00147153 -->

    <owl:NamedIndividual rdf:about="http://purl.obolibrary.org/obo/GAZ_00147153">
        <obo:RO_0001025 rdf:resource="http://purl.obolibrary.org/obo/GAZ_00147152"/>
        <obo:IAO_0000115>A bay on Cape Foulwind.</obo:IAO_0000115>
        <oboInOwl:hasOBONamespace>GAZ</oboInOwl:hasOBONamespace>
        <oboInOwl:id>GAZ:00147153</oboInOwl:id>
        <rdfs:label>Tauranga Bay</rdfs:label>
    </owl:NamedIndividual>
    


    <!-- http://purl.obolibrary.org/obo/GAZ_00147154 -->

    <owl:NamedIndividual rdf:about="http://purl.obolibrary.org/obo/GAZ_00147154">
        <obo:RO_0001025 rdf:resource="http://purl.obolibrary.org/obo/GAZ_00010248"/>
        <obo:IAO_0000115>A prominent headland on the northeastern coast of New Zealand&apos;s North island. It is located 30 km northeast of Tuaheni Point and 20 km south of Tolaga Bay.</obo:IAO_0000115>
        <oboInOwl:hasOBONamespace>GAZ</oboInOwl:hasOBONamespace>
        <oboInOwl:id>GAZ:00147154</oboInOwl:id>
        <rdfs:label>Gable End Foreland</rdfs:label>
    </owl:NamedIndividual>
    


    <!-- http://purl.obolibrary.org/obo/GAZ_00147155 -->

    <owl:NamedIndividual rdf:about="http://purl.obolibrary.org/obo/GAZ_00147155">
        <obo:RO_0001025 rdf:resource="http://purl.obolibrary.org/obo/GAZ_00008568"/>
        <obo:IAO_0000115>A peninsula in Marlborough, in the South Island of New Zealand. It lies between Queen Charlotte Sound and Cook Strait.</obo:IAO_0000115>
        <oboInOwl:hasOBONamespace>GAZ</oboInOwl:hasOBONamespace>
        <oboInOwl:id>GAZ:00147155</oboInOwl:id>
        <rdfs:label>Cape Jackson</rdfs:label>
    </owl:NamedIndividual>
    


    <!-- http://purl.obolibrary.org/obo/GAZ_00147156 -->

    <owl:NamedIndividual rdf:about="http://purl.obolibrary.org/obo/GAZ_00147156">
        <rdf:type rdf:resource="http://purl.obolibrary.org/obo/ENVO_00000305"/>
        <obo:RO_0001025 rdf:resource="http://purl.obolibrary.org/obo/GAZ_00008563"/>
        <obo:IAO_0000115>A headland on the West Coast of New Zealand&apos;s South Island, overlooking the Tasman Sea. It is located in Kahurangi National Park between Karamea and Farewell Spit.</obo:IAO_0000115>
        <oboInOwl:hasOBONamespace>GAZ</oboInOwl:hasOBONamespace>
        <oboInOwl:id>GAZ:00147156</oboInOwl:id>
        <rdfs:label>Kahurangi Point</rdfs:label>
    </owl:NamedIndividual>
    


    <!-- http://purl.obolibrary.org/obo/GAZ_00147157 -->

    <owl:NamedIndividual rdf:about="http://purl.obolibrary.org/obo/GAZ_00147157">
        <obo:RO_0001025 rdf:resource="http://purl.obolibrary.org/obo/GAZ_00004768"/>
        <obo:IAO_0000115>A prominent landmark on the coast of Otago, New Zealand. Located within the city of Dunedin, this rocky headland juts into the Pacific Ocean at the eastern end of the city&apos;s main beach, Saint Kilda Beach.</obo:IAO_0000115>
        <oboInOwl:hasOBONamespace>GAZ</oboInOwl:hasOBONamespace>
        <oboInOwl:id>GAZ:00147157</oboInOwl:id>
        <rdfs:label>Lawyer&apos;s Head</rdfs:label>
    </owl:NamedIndividual>
    


    <!-- http://purl.obolibrary.org/obo/GAZ_00147158 -->

    <owl:NamedIndividual rdf:about="http://purl.obolibrary.org/obo/GAZ_00147158">
        <rdf:type rdf:resource="http://purl.obolibrary.org/obo/ENVO_00000305"/>
        <obo:RO_0001025 rdf:resource="http://purl.obolibrary.org/obo/GAZ_00146864"/>
        <obo:IAO_0000115>A headland at the N end of the Catlins Coast.</obo:IAO_0000115>
        <oboInOwl:hasOBONamespace>GAZ</oboInOwl:hasOBONamespace>
        <oboInOwl:id>GAZ:00147158</oboInOwl:id>
        <rdfs:label>Nugget Point</rdfs:label>
    </owl:NamedIndividual>
    


    <!-- http://purl.obolibrary.org/obo/GAZ_00147159 -->

    <owl:NamedIndividual rdf:about="http://purl.obolibrary.org/obo/GAZ_00147159">
        <obo:RO_0001025 rdf:resource="http://purl.obolibrary.org/obo/GAZ_00146864"/>
        <obo:IAO_0000115>Rocky small islands that surround Nugget Point.</obo:IAO_0000115>
        <oboInOwl:hasOBONamespace>GAZ</oboInOwl:hasOBONamespace>
        <oboInOwl:id>GAZ:00147159</oboInOwl:id>
        <rdfs:label>The Nuggets</rdfs:label>
    </owl:NamedIndividual>
    


    <!-- http://purl.obolibrary.org/obo/GAZ_00147160 -->

    <owl:NamedIndividual rdf:about="http://purl.obolibrary.org/obo/GAZ_00147160">
        <obo:RO_0001025 rdf:resource="http://purl.obolibrary.org/obo/GAZ_00004760"/>
        <obo:IAO_0000115>The two promontories that form the entrance to the Manukau Harbour - one of the two harbours of Auckland in New Zealand.</obo:IAO_0000115>
        <oboInOwl:hasOBONamespace>GAZ</oboInOwl:hasOBONamespace>
        <oboInOwl:id>GAZ:00147160</oboInOwl:id>
        <rdfs:label>Manukau Heads</rdfs:label>
    </owl:NamedIndividual>
    


    <!-- http://purl.obolibrary.org/obo/GAZ_00147161 -->

    <owl:NamedIndividual rdf:about="http://purl.obolibrary.org/obo/GAZ_00147161">
        <obo:RO_0001025 rdf:resource="http://purl.obolibrary.org/obo/GAZ_00147160"/>
        <obo:IAO_0000115>The S of the Manukau Heads.</obo:IAO_0000115>
        <oboInOwl:hasOBONamespace>GAZ</oboInOwl:hasOBONamespace>
        <oboInOwl:id>GAZ:00147161</oboInOwl:id>
        <rdfs:label>South Head</rdfs:label>
    </owl:NamedIndividual>
    


    <!-- http://purl.obolibrary.org/obo/GAZ_00147162 -->

    <owl:NamedIndividual rdf:about="http://purl.obolibrary.org/obo/GAZ_00147162">
        <obo:RO_0001025 rdf:resource="http://purl.obolibrary.org/obo/GAZ_00147160"/>
        <obo:IAO_0000115>The N of the Manukau Heads.</obo:IAO_0000115>
        <oboInOwl:hasOBONamespace>GAZ</oboInOwl:hasOBONamespace>
        <oboInOwl:id>GAZ:00147162</oboInOwl:id>
        <rdfs:label>Burnett Head</rdfs:label>
    </owl:NamedIndividual>
    


    <!-- http://purl.obolibrary.org/obo/GAZ_00147163 -->

    <owl:NamedIndividual rdf:about="http://purl.obolibrary.org/obo/GAZ_00147163">
        <rdf:type rdf:resource="http://purl.obolibrary.org/obo/ENVO_00000305"/>
        <obo:RO_0001025 rdf:resource="http://purl.obolibrary.org/obo/GAZ_00008569"/>
        <obo:IAO_0000115>A head of the Whangarei Harbour, near Whangarei, New Zealand, lying close to the northern tip of Bream Bay.</obo:IAO_0000115>
        <oboInOwl:hasOBONamespace>GAZ</oboInOwl:hasOBONamespace>
        <oboInOwl:id>GAZ:00147163</oboInOwl:id>
        <rdfs:label>Marsden Point</rdfs:label>
    </owl:NamedIndividual>
    


    <!-- http://purl.obolibrary.org/obo/GAZ_00147164 -->

    <owl:NamedIndividual rdf:about="http://purl.obolibrary.org/obo/GAZ_00147164">
        <obo:RO_0001025 rdf:resource="http://purl.obolibrary.org/obo/GAZ_00008569"/>
        <obo:IAO_0000115>A bay at the south head of Whangarei Harbour in Northland, New Zealand. The western side of Marsden Bay is a coastal community called One Tree Point, and the eastern side is the industrial development of Marsden Point.</obo:IAO_0000115>
        <oboInOwl:hasOBONamespace>GAZ</oboInOwl:hasOBONamespace>
        <oboInOwl:id>GAZ:00147164</oboInOwl:id>
        <rdfs:label>Marsden Bay</rdfs:label>
    </owl:NamedIndividual>
    


    <!-- http://purl.obolibrary.org/obo/GAZ_00147165 -->

    <owl:NamedIndividual rdf:about="http://purl.obolibrary.org/obo/GAZ_00147165">
        <obo:RO_0001025 rdf:resource="http://purl.obolibrary.org/obo/GAZ_00030194"/>
        <obo:IAO_0000115>A volcanic headland within North Shore City, New Zealand, in the suburb of Devonport at the east end of the Waitemata Harbour (Auckland&apos;s harbour).</obo:IAO_0000115>
        <oboInOwl:hasOBONamespace>GAZ</oboInOwl:hasOBONamespace>
        <oboInOwl:id>GAZ:00147165</oboInOwl:id>
        <rdfs:label>North Head</rdfs:label>
    </owl:NamedIndividual>
    


    <!-- http://purl.obolibrary.org/obo/GAZ_00147166 -->

    <owl:NamedIndividual rdf:about="http://purl.obolibrary.org/obo/GAZ_00147166">
        <obo:RO_0001025 rdf:resource="http://purl.obolibrary.org/obo/GAZ_00008565"/>
        <obo:IAO_0000115>The southwesternmost point of the North Island of New Zealand. The cape is located 16 km to the west of Wellington, the capital city of New Zealand. Ohau Point, located on the northern tip of Cape Terawhiti and, along with Perano Head on Arapawa Island in the Marlborough Sounds, marks the narrowest part of Cook Strait.</obo:IAO_0000115>
        <oboInOwl:hasOBONamespace>GAZ</oboInOwl:hasOBONamespace>
        <oboInOwl:id>GAZ:00147166</oboInOwl:id>
        <rdfs:label>Cape Terawhiti</rdfs:label>
    </owl:NamedIndividual>
    


    <!-- http://purl.obolibrary.org/obo/GAZ_00147167 -->

    <owl:NamedIndividual rdf:about="http://purl.obolibrary.org/obo/GAZ_00147167">
        <rdf:type rdf:resource="http://purl.obolibrary.org/obo/ENVO_00000305"/>
        <obo:RO_0001025 rdf:resource="http://purl.obolibrary.org/obo/GAZ_00147166"/>
        <obo:IAO_0000115>A headland located on the northern tip of Cape Terawhiti.</obo:IAO_0000115>
        <oboInOwl:hasOBONamespace>GAZ</oboInOwl:hasOBONamespace>
        <oboInOwl:id>GAZ:00147167</oboInOwl:id>
        <rdfs:label>Ohau Point</rdfs:label>
    </owl:NamedIndividual>
    


    <!-- http://purl.obolibrary.org/obo/GAZ_00147168 -->

    <owl:NamedIndividual rdf:about="http://purl.obolibrary.org/obo/GAZ_00147168">
        <rdf:type rdf:resource="http://purl.obolibrary.org/obo/ENVO_00000305"/>
        <obo:RO_0001025 rdf:resource="http://purl.obolibrary.org/obo/GAZ_00008565"/>
        <obo:IAO_0000115>A headland on the southern coast of New Zealand&apos;s North Island and the southernmost point of the North Island. It is located at the eastern end of Palliser Bay, 50 km southeast of Wellington.</obo:IAO_0000115>
        <oboInOwl:hasOBONamespace>GAZ</oboInOwl:hasOBONamespace>
        <oboInOwl:id>GAZ:00147168</oboInOwl:id>
        <rdfs:label>Cape Palliser</rdfs:label>
    </owl:NamedIndividual>
    


    <!-- http://purl.obolibrary.org/obo/GAZ_00147169 -->

    <owl:NamedIndividual rdf:about="http://purl.obolibrary.org/obo/GAZ_00147169">
        <obo:RO_0001025 rdf:resource="http://purl.obolibrary.org/obo/GAZ_00147168"/>
        <obo:IAO_0000115>A geological formation near the eastern end of Palliser Bay at the southern end of the North Island of New Zealand.</obo:IAO_0000115>
        <oboInOwl:hasOBONamespace>GAZ</oboInOwl:hasOBONamespace>
        <oboInOwl:id>GAZ:00147169</oboInOwl:id>
        <rdfs:label>Kupe&apos;s Sail</rdfs:label>
    </owl:NamedIndividual>
    


    <!-- http://purl.obolibrary.org/obo/GAZ_00147170 -->

    <owl:NamedIndividual rdf:about="http://purl.obolibrary.org/obo/GAZ_00147170">
        <rdf:type rdf:resource="http://purl.obolibrary.org/obo/ENVO_00000305"/>
        <obo:RO_0001025 rdf:resource="http://purl.obolibrary.org/obo/GAZ_00047047"/>
        <obo:IAO_0000115>A headland located in the far southwest of the South Island of New Zealand. It lies within Fiordland National Park on the southern head of Preservation Inlet.</obo:IAO_0000115>
        <oboInOwl:hasOBONamespace>GAZ</oboInOwl:hasOBONamespace>
        <oboInOwl:id>GAZ:00147170</oboInOwl:id>
        <rdfs:label>Puysegur Point</rdfs:label>
    </owl:NamedIndividual>
    


    <!-- http://purl.obolibrary.org/obo/GAZ_00147171 -->

    <owl:NamedIndividual rdf:about="http://purl.obolibrary.org/obo/GAZ_00147171">
        <obo:RO_0001025 rdf:resource="http://purl.obolibrary.org/obo/GAZ_00010248"/>
        <obo:IAO_0000115>The eastern extremity of the Bay of Plenty in New Zealand&apos;s North Island. It is located 90 km northeast off Whakatane and 50 km west of East Cape.</obo:IAO_0000115>
        <oboInOwl:hasOBONamespace>GAZ</oboInOwl:hasOBONamespace>
        <oboInOwl:id>GAZ:00147171</oboInOwl:id>
        <rdfs:label>Cape Runaway</rdfs:label>
    </owl:NamedIndividual>
    


    <!-- http://purl.obolibrary.org/obo/GAZ_00147173 -->

    <owl:NamedIndividual rdf:about="http://purl.obolibrary.org/obo/GAZ_00147173">
        <obo:RO_0001025 rdf:resource="http://purl.obolibrary.org/obo/GAZ_00146864"/>
        <obo:IAO_0000115>A rocky headland on the south coast of the South Island of New Zealand. It is located 25 km east of Waikawa, at the western end of a bay (Tautuku Bay) in the area known as the Catlins.</obo:IAO_0000115>
        <oboInOwl:hasOBONamespace>GAZ</oboInOwl:hasOBONamespace>
        <oboInOwl:id>GAZ:00147173</oboInOwl:id>
        <rdfs:label>Tautuku Peninsula</rdfs:label>
    </owl:NamedIndividual>
    


    <!-- http://purl.obolibrary.org/obo/GAZ_00147174 -->

    <owl:NamedIndividual rdf:about="http://purl.obolibrary.org/obo/GAZ_00147174">
        <obo:RO_0001025 rdf:resource="http://purl.obolibrary.org/obo/GAZ_00008565"/>
        <obo:IAO_0000115>A rugged coastal landform in Wellington New Zealand. It is located adjacent to Princess Bay, between Houghton Bay to the west and Lyall Bay to the east on the south coast of Wellington.</obo:IAO_0000115>
        <oboInOwl:hasOBONamespace>GAZ</oboInOwl:hasOBONamespace>
        <oboInOwl:id>GAZ:00147174</oboInOwl:id>
        <rdfs:label>Te Raekaihau Point</rdfs:label>
    </owl:NamedIndividual>
    


    <!-- http://purl.obolibrary.org/obo/GAZ_00147175 -->

    <owl:NamedIndividual rdf:about="http://purl.obolibrary.org/obo/GAZ_00147175">
        <rdf:type rdf:resource="http://purl.obolibrary.org/obo/ENVO_00000305"/>
        <obo:RO_0001025 rdf:resource="http://purl.obolibrary.org/obo/GAZ_00010248"/>
        <obo:IAO_0000115>A headland on the east coast of the North island of New Zealand. It marks the northernmost point of Poverty Bay, and is located close to the city of Gisborne.</obo:IAO_0000115>
        <oboInOwl:hasOBONamespace>GAZ</oboInOwl:hasOBONamespace>
        <oboInOwl:id>GAZ:00147175</oboInOwl:id>
        <rdfs:label>Tuaheni Point</rdfs:label>
    </owl:NamedIndividual>
    


    <!-- http://purl.obolibrary.org/obo/GAZ_00147176 -->

    <owl:NamedIndividual rdf:about="http://purl.obolibrary.org/obo/GAZ_00147176">
        <rdf:type rdf:resource="http://purl.obolibrary.org/obo/ENVO_00000305"/>
        <obo:RO_0001025 rdf:resource="http://purl.obolibrary.org/obo/GAZ_00008565"/>
        <obo:RO_0001025 rdf:resource="http://purl.obolibrary.org/obo/GAZ_00147144"/>
        <obo:IAO_0000115>A headland on the southern coast of New Zealand&apos;s North Island. It is located at the western end of Palliser Bay, 20 km southeast of Wellington, at the southern end of the Rimutaka Ranges.</obo:IAO_0000115>
        <oboInOwl:hasOBONamespace>GAZ</oboInOwl:hasOBONamespace>
        <oboInOwl:id>GAZ:00147176</oboInOwl:id>
        <rdfs:label>Turakirae Head</rdfs:label>
    </owl:NamedIndividual>
    


    <!-- http://purl.obolibrary.org/obo/GAZ_00147177 -->

    <owl:NamedIndividual rdf:about="http://purl.obolibrary.org/obo/GAZ_00147177">
        <obo:RO_0001025 rdf:resource="http://purl.obolibrary.org/obo/GAZ_00146864"/>
        <obo:IAO_0000115>A rocky promontory on the south coast of the South Island of New Zealand. It is located 10 km (6 miles) southeast of the mouth of the Mataura River, at the extreme southwestern end of the area known as the Catlins.</obo:IAO_0000115>
        <oboInOwl:hasOBONamespace>GAZ</oboInOwl:hasOBONamespace>
        <oboInOwl:id>GAZ:00147177</oboInOwl:id>
        <rdfs:label>Waipapa Point</rdfs:label>
    </owl:NamedIndividual>
    


    <!-- http://purl.obolibrary.org/obo/GAZ_00147178 -->

    <owl:NamedIndividual rdf:about="http://purl.obolibrary.org/obo/GAZ_00147178">
        <obo:RO_0001025 rdf:resource="http://purl.obolibrary.org/obo/GAZ_00030217"/>
        <obo:RO_0001025 rdf:resource="http://purl.obolibrary.org/obo/GAZ_00088598"/>
        <obo:IAO_0000115>A 12 km long glacier located in Westland National Park on the West Coast of New Zealand&apos;s South Island.</obo:IAO_0000115>
        <oboInOwl:hasOBONamespace>GAZ</oboInOwl:hasOBONamespace>
        <oboInOwl:id>GAZ:00147178</oboInOwl:id>
        <rdfs:label>Fox Glacier</rdfs:label>
    </owl:NamedIndividual>
    


    <!-- http://purl.obolibrary.org/obo/GAZ_00147179 -->

    <owl:NamedIndividual rdf:about="http://purl.obolibrary.org/obo/GAZ_00147179">
        <obo:RO_0001025 rdf:resource="http://purl.obolibrary.org/obo/GAZ_00030217"/>
        <obo:RO_0001025 rdf:resource="http://purl.obolibrary.org/obo/GAZ_00088598"/>
        <obo:IAO_0000115>A12 km long[ glacier located in Westland National Park on the West Coast of New Zealand&apos;s South Island.</obo:IAO_0000115>
        <oboInOwl:hasOBONamespace>GAZ</oboInOwl:hasOBONamespace>
        <oboInOwl:id>GAZ:00147179</oboInOwl:id>
        <rdfs:label>Franz Josef Glacier</rdfs:label>
    </owl:NamedIndividual>
    


    <!-- http://purl.obolibrary.org/obo/GAZ_00147180 -->

    <owl:NamedIndividual rdf:about="http://purl.obolibrary.org/obo/GAZ_00147180">
        <obo:RO_0001025 rdf:resource="http://purl.obolibrary.org/obo/GAZ_00008562"/>
        <obo:IAO_0000115>An area bounded by the foothills of the Southern Alps and the east coast of the South Island of New Zealand. They are centred to the south of the city of Christchurch in the Canterbury region. Their northern extremes are at the foot of the Hundalee Hills in the Hurunui District, and in the south they merge into the plains of North Otago beyond the Waitaki River.</obo:IAO_0000115>
        <oboInOwl:hasOBONamespace>GAZ</oboInOwl:hasOBONamespace>
        <oboInOwl:id>GAZ:00147180</oboInOwl:id>
        <rdfs:label>Canterbury Plains</rdfs:label>
    </owl:NamedIndividual>
    


    <!-- http://purl.obolibrary.org/obo/GAZ_00147181 -->

    <owl:NamedIndividual rdf:about="http://purl.obolibrary.org/obo/GAZ_00147181">
        <obo:RO_0001025 rdf:resource="http://purl.obolibrary.org/obo/GAZ_00029965"/>
        <obo:IAO_0000115>A peninsula located in the northeast of New Zealand&apos;s South Island. It protrudes 5 km into the Pacific Ocean. The town of Kaikoura is located on the north shore of the peninsula.</obo:IAO_0000115>
        <oboInOwl:hasOBONamespace>GAZ</oboInOwl:hasOBONamespace>
        <oboInOwl:id>GAZ:00147181</oboInOwl:id>
        <rdfs:label>Kaikoura Peninsula</rdfs:label>
    </owl:NamedIndividual>
    


    <!-- http://purl.obolibrary.org/obo/GAZ_00147182 -->

    <owl:NamedIndividual rdf:about="http://purl.obolibrary.org/obo/GAZ_00147182">
        <obo:RO_0001025 rdf:resource="http://purl.obolibrary.org/obo/GAZ_00012589"/>
        <obo:IAO_0000115>A rocky headland1 km to the south of Oamaru, New Zealand.</obo:IAO_0000115>
        <oboInOwl:hasOBONamespace>GAZ</oboInOwl:hasOBONamespace>
        <oboInOwl:id>GAZ:00147182</oboInOwl:id>
        <rdfs:label>Cape Wanbrow</rdfs:label>
    </owl:NamedIndividual>
    


    <!-- http://purl.obolibrary.org/obo/GAZ_00147183 -->

    <owl:NamedIndividual rdf:about="http://purl.obolibrary.org/obo/GAZ_00147183">
        <obo:RO_0001025 rdf:resource="http://purl.obolibrary.org/obo/GAZ_00047047"/>
        <obo:IAO_0000115>The westernmost point in the main chain of islands of New Zealand. It is located in the far southwest of the South Island, within Fiordland National Park, between Dusky Sound and Chalky Inlet.</obo:IAO_0000115>
        <oboInOwl:hasOBONamespace>GAZ</oboInOwl:hasOBONamespace>
        <oboInOwl:id>GAZ:00147183</oboInOwl:id>
        <rdfs:label>West Cape</rdfs:label>
    </owl:NamedIndividual>
    


    <!-- http://purl.obolibrary.org/obo/GAZ_00147184 -->

    <owl:NamedIndividual rdf:about="http://purl.obolibrary.org/obo/GAZ_00147184">
        <rdf:type rdf:resource="http://purl.obolibrary.org/obo/ENVO_00000305"/>
        <obo:RO_0001025 rdf:resource="http://purl.obolibrary.org/obo/GAZ_00030228"/>
        <obo:IAO_0000115>A headland at the entrance to Okains Bay on Banks Peninsula.</obo:IAO_0000115>
        <oboInOwl:hasOBONamespace>GAZ</oboInOwl:hasOBONamespace>
        <oboInOwl:id>GAZ:00147184</oboInOwl:id>
        <rdfs:label>West Head</rdfs:label>
    </owl:NamedIndividual>
    


    <!-- http://purl.obolibrary.org/obo/GAZ_00147185 -->

    <owl:NamedIndividual rdf:about="http://purl.obolibrary.org/obo/GAZ_00147185">
        <obo:RO_0001025 rdf:resource="http://purl.obolibrary.org/obo/GAZ_00008568"/>
        <obo:IAO_0000115>The headland at the end of a peninsula on the northern shore of Queen Charlotte Sound.</obo:IAO_0000115>
        <oboInOwl:hasOBONamespace>GAZ</oboInOwl:hasOBONamespace>
        <oboInOwl:id>GAZ:00147185</oboInOwl:id>
        <rdfs:label>West Head [Queen Charlotte Sound]</rdfs:label>
    </owl:NamedIndividual>
    


    <!-- http://purl.obolibrary.org/obo/GAZ_00147186 -->

    <owl:NamedIndividual rdf:about="http://purl.obolibrary.org/obo/GAZ_00147186">
        <obo:RO_0001025 rdf:resource="http://purl.obolibrary.org/obo/GAZ_00008568"/>
        <obo:IAO_0000115>A rocky headland at the entrance to Tory Channel.</obo:IAO_0000115>
        <oboInOwl:hasOBONamespace>GAZ</oboInOwl:hasOBONamespace>
        <oboInOwl:id>GAZ:00147186</oboInOwl:id>
        <rdfs:label>West Head [Tory Channel]</rdfs:label>
    </owl:NamedIndividual>
    


    <!-- http://purl.obolibrary.org/obo/GAZ_00147187 -->

    <owl:NamedIndividual rdf:about="http://purl.obolibrary.org/obo/GAZ_00147187">
        <rdf:type rdf:resource="http://purl.obolibrary.org/obo/ENVO_00000305"/>
        <obo:RO_0001025 rdf:resource="http://purl.obolibrary.org/obo/GAZ_00010248"/>
        <obo:IAO_0000115>A headland at the southern end of Poverty Bay in New Zealand&apos;s North Island.</obo:IAO_0000115>
        <oboInOwl:hasOBONamespace>GAZ</oboInOwl:hasOBONamespace>
        <oboInOwl:id>GAZ:00147187</oboInOwl:id>
        <rdfs:label>Young Nick&apos;s Head</rdfs:label>
    </owl:NamedIndividual>
    


    <!-- http://purl.obolibrary.org/obo/GAZ_00147188 -->

    <owl:NamedIndividual rdf:about="http://purl.obolibrary.org/obo/GAZ_00147188">
        <rdf:type rdf:resource="http://purl.obolibrary.org/obo/ENVO_00000305"/>
        <obo:RO_0001025 rdf:resource="http://purl.obolibrary.org/obo/GAZ_00008569"/>
        <obo:IAO_0000115>A headland on the east coast of Northland in the North Island of New Zealand. Located at the end of a 30 km peninsula, the head juts into the Pacific Ocean to the southeast of Whangarei. The Hen and Chicken Islands are located off the headland at a distance of 12 km.</obo:IAO_0000115>
        <oboInOwl:hasOBONamespace>GAZ</oboInOwl:hasOBONamespace>
        <oboInOwl:id>GAZ:00147188</oboInOwl:id>
        <rdfs:label>Bream Head</rdfs:label>
    </owl:NamedIndividual>
    


    <!-- http://purl.obolibrary.org/obo/GAZ_00147189 -->

    <owl:NamedIndividual rdf:about="http://purl.obolibrary.org/obo/GAZ_00147189">
        <rdf:type rdf:resource="http://purl.obolibrary.org/obo/ENVO_00000305"/>
        <obo:RO_0001025 rdf:resource="http://purl.obolibrary.org/obo/GAZ_00010256"/>
        <obo:IAO_0000115>A headland at the southeastern extremity of Hawke Bay on the east coast of New Zealand&apos;s North Island. It is located 20 km southeast of the city of Napier. The promontory sits at the end of an eight km long peninsula which protrudes into the Pacific Ocean.</obo:IAO_0000115>
        <oboInOwl:hasOBONamespace>GAZ</oboInOwl:hasOBONamespace>
        <oboInOwl:id>GAZ:00147189</oboInOwl:id>
        <rdfs:label>Cape Kidnappers</rdfs:label>
    </owl:NamedIndividual>
    


    <!-- http://purl.obolibrary.org/obo/GAZ_00147190 -->

    <owl:NamedIndividual rdf:about="http://purl.obolibrary.org/obo/GAZ_00147190">
        <obo:RO_0001025 rdf:resource="http://purl.obolibrary.org/obo/GAZ_00004772"/>
        <obo:IAO_0000115>A prominent headland on the east coast of New Zealand&apos;s North Island, part way between Hawke Bay and Cook Strait, between the mouths of the Porangahau and Akitio Rivers.</obo:IAO_0000115>
        <oboInOwl:hasOBONamespace>GAZ</oboInOwl:hasOBONamespace>
        <oboInOwl:id>GAZ:00147190</oboInOwl:id>
        <rdfs:label>Cape Turnagain</rdfs:label>
    </owl:NamedIndividual>
    


    <!-- http://purl.obolibrary.org/obo/GAZ_00147191 -->

    <owl:NamedIndividual rdf:about="http://purl.obolibrary.org/obo/GAZ_00147191">
        <obo:RO_0001025 rdf:resource="http://purl.obolibrary.org/obo/GAZ_00009534"/>
        <obo:IAO_0000115>A peninsula in the west of the city of Auckland in the north of New Zealand. It is located 5 km to the west of the city centre on the southern shore of the Waitemata Harbour.</obo:IAO_0000115>
        <oboInOwl:hasOBONamespace>GAZ</oboInOwl:hasOBONamespace>
        <oboInOwl:id>GAZ:00147191</oboInOwl:id>
        <rdfs:label>Point Chevalier</rdfs:label>
    </owl:NamedIndividual>
    


    <!-- http://purl.obolibrary.org/obo/GAZ_00147192 -->

    <owl:NamedIndividual rdf:about="http://purl.obolibrary.org/obo/GAZ_00147192">
        <obo:RO_0001025 rdf:resource="http://purl.obolibrary.org/obo/GAZ_00008569"/>
        <obo:IAO_0000115>A peninsula on the northern Kaipara Harbour in Northland, New Zealand. The Peninsula runs in the north west to south east direction and is approximately 55 km long. The width varies from about 5.4 km to about 14 km, with the widest part of the peninsula near its southern end. The Tasman Sea is to the west, and the Kaipara Harbour is to the south. The Wairoa River and Kaipara Harbour are to the east.</obo:IAO_0000115>
        <oboInOwl:hasOBONamespace>GAZ</oboInOwl:hasOBONamespace>
        <oboInOwl:id>GAZ:00147192</oboInOwl:id>
        <rdfs:label>Pouto Peninsula</rdfs:label>
    </owl:NamedIndividual>
    


    <!-- http://purl.obolibrary.org/obo/GAZ_00147193 -->

    <owl:NamedIndividual rdf:about="http://purl.obolibrary.org/obo/GAZ_00147193">
        <obo:RO_0001025 rdf:resource="http://purl.obolibrary.org/obo/GAZ_00029928"/>
        <obo:IAO_0000115>A peninsula on the northwest side of the Bay of Islands in Northland, New Zealand.</obo:IAO_0000115>
        <oboInOwl:hasOBONamespace>GAZ</oboInOwl:hasOBONamespace>
        <oboInOwl:id>GAZ:00147193</oboInOwl:id>
        <rdfs:label>Purerua Peninsula</rdfs:label>
    </owl:NamedIndividual>
    


    <!-- http://purl.obolibrary.org/obo/GAZ_00147194 -->

    <owl:NamedIndividual rdf:about="http://purl.obolibrary.org/obo/GAZ_00147194">
        <obo:RO_0001025 rdf:resource="http://purl.obolibrary.org/obo/GAZ_00004760"/>
        <obo:IAO_0000115>A peninsula projecting into the Hauraki Gulf from the east coast of the much larger North Auckland Peninsula of New Zealand. It separates Omaha Bay to the north from Kawau Bay and Kawau Island to the south.</obo:IAO_0000115>
        <oboInOwl:hasOBONamespace>GAZ</oboInOwl:hasOBONamespace>
        <oboInOwl:id>GAZ:00147194</oboInOwl:id>
        <rdfs:label>Tawharanui Peninsula</rdfs:label>
    </owl:NamedIndividual>
    


    <!-- http://purl.obolibrary.org/obo/GAZ_00147195 -->

    <owl:NamedIndividual rdf:about="http://purl.obolibrary.org/obo/GAZ_00147195">
        <obo:RO_0001025 rdf:resource="http://purl.obolibrary.org/obo/GAZ_00147196"/>
        <obo:IAO_0000115>A peninsula at the entrance to Bluff Harbour on the southern coast of the South Island of New Zealand. A spit which extends from the western end of the Awarua Plain, it lies between Awarua Bay to the north and Foveaux Strait to the south.</obo:IAO_0000115>
        <oboInOwl:hasOBONamespace>GAZ</oboInOwl:hasOBONamespace>
        <oboInOwl:id>GAZ:00147195</oboInOwl:id>
        <rdfs:label>Tiwai Point</rdfs:label>
    </owl:NamedIndividual>
    


    <!-- http://purl.obolibrary.org/obo/GAZ_00147196 -->

    <owl:NamedIndividual rdf:about="http://purl.obolibrary.org/obo/GAZ_00147196">
        <obo:RO_0001025 rdf:resource="http://purl.obolibrary.org/obo/GAZ_00008572"/>
        <obo:IAO_0000115>A large area of wetland to the east of Bluff, New Zealand. Covering an area of around 600 km2, the plain stretches for 35 km along the coast of Foveaux Strait. This stretch of coast includes the peninsula of Tiwai Point, Awarua Bay, the Waituna Lagoon, and Toetoes Bay.</obo:IAO_0000115>
        <oboInOwl:hasOBONamespace>GAZ</oboInOwl:hasOBONamespace>
        <oboInOwl:id>GAZ:00147196</oboInOwl:id>
        <rdfs:label>Awarua Plain</rdfs:label>
    </owl:NamedIndividual>
    


    <!-- http://purl.obolibrary.org/obo/GAZ_00147197 -->

    <owl:NamedIndividual rdf:about="http://purl.obolibrary.org/obo/GAZ_00147197">
        <obo:RO_0001025 rdf:resource="http://purl.obolibrary.org/obo/GAZ_00004760"/>
        <obo:IAO_0000115>A peninsula located in the northern North Island of New Zealand, close to the base of the North Auckland Peninsula.</obo:IAO_0000115>
        <oboInOwl:hasOBONamespace>GAZ</oboInOwl:hasOBONamespace>
        <oboInOwl:id>GAZ:00147197</oboInOwl:id>
        <rdfs:label>Whangaparaoa Peninsula</rdfs:label>
    </owl:NamedIndividual>
    


    <!-- http://purl.obolibrary.org/obo/GAZ_00147198 -->

    <owl:NamedIndividual rdf:about="http://purl.obolibrary.org/obo/GAZ_00147198">
        <obo:RO_0001025 rdf:resource="http://purl.obolibrary.org/obo/GAZ_00147196"/>
        <obo:IAO_0000115>A bay.</obo:IAO_0000115>
        <oboInOwl:hasOBONamespace>GAZ</oboInOwl:hasOBONamespace>
        <oboInOwl:id>GAZ:00147198</oboInOwl:id>
        <rdfs:label>Awarua Bay</rdfs:label>
    </owl:NamedIndividual>
    


    <!-- http://purl.obolibrary.org/obo/GAZ_00147199 -->

    <owl:NamedIndividual rdf:about="http://purl.obolibrary.org/obo/GAZ_00147199">
        <rdf:type rdf:resource="http://purl.obolibrary.org/obo/ENVO_00000305"/>
        <obo:RO_0001025 rdf:resource="http://purl.obolibrary.org/obo/GAZ_00008568"/>
        <obo:IAO_0000115>A headland that marks the eastern limit of the Wilson Bay Farm and the southern approach to Tawhitinui Reach in Pelorus Sound, part of the Marlborough Sounds Maritime Park at the top of the South Island of New Zealand.</obo:IAO_0000115>
        <oboInOwl:hasOBONamespace>GAZ</oboInOwl:hasOBONamespace>
        <oboInOwl:id>GAZ:00147199</oboInOwl:id>
        <rdfs:label>Tawero Point</rdfs:label>
    </owl:NamedIndividual>
    


    <!-- http://purl.obolibrary.org/obo/GAZ_00147200 -->

    <owl:NamedIndividual rdf:about="http://purl.obolibrary.org/obo/GAZ_00147200">
        <obo:RO_0001025 rdf:resource="http://purl.obolibrary.org/obo/GAZ_00053838"/>
        <obo:IAO_0000115>A basin occupying a volcanic crater within the Auckland Volcanic Field in New Zealand. It is located to the south of Panmure town centre.</obo:IAO_0000115>
        <oboInOwl:hasOBONamespace>GAZ</oboInOwl:hasOBONamespace>
        <oboInOwl:id>GAZ:00147200</oboInOwl:id>
        <rdfs:label>Panmure Basin</rdfs:label>
    </owl:NamedIndividual>
    


    <!-- http://purl.obolibrary.org/obo/GAZ_00147201 -->

    <owl:NamedIndividual rdf:about="http://purl.obolibrary.org/obo/GAZ_00147201">
        <obo:RO_0001025 rdf:resource="http://purl.obolibrary.org/obo/GAZ_00008562"/>
        <obo:IAO_0000115>A long finger of land which extends along the coast of Canterbury in the South Island of New Zealand. It runs southwest from Banks Peninsula for 25 km, and separates the shallow Lake Ellesmere from the Canterbury Bight and Pacific Ocean.</obo:IAO_0000115>
        <oboInOwl:hasOBONamespace>GAZ</oboInOwl:hasOBONamespace>
        <oboInOwl:id>GAZ:00147201</oboInOwl:id>
        <rdfs:label>Kaitorete Spit</rdfs:label>
    </owl:NamedIndividual>
    


    <!-- http://purl.obolibrary.org/obo/GAZ_00147202 -->

    <owl:NamedIndividual rdf:about="http://purl.obolibrary.org/obo/GAZ_00147202">
        <obo:RO_0001025 rdf:resource="http://purl.obolibrary.org/obo/GAZ_00147147"/>
        <obo:IAO_0000115>The southernmost point of the Mahia Peninsula, in the northern Hawke&apos;s Bay Region of New Zealand&apos;s eastern North Island.</obo:IAO_0000115>
        <oboInOwl:hasOBONamespace>GAZ</oboInOwl:hasOBONamespace>
        <oboInOwl:id>GAZ:00147202</oboInOwl:id>
        <rdfs:label>Ahuriri Point</rdfs:label>
    </owl:NamedIndividual>
    


    <!-- http://purl.obolibrary.org/obo/GAZ_00147203 -->

    <owl:NamedIndividual rdf:about="http://purl.obolibrary.org/obo/GAZ_00147203">
        <obo:RO_0001025 rdf:resource="http://purl.obolibrary.org/obo/GAZ_00146864"/>
        <obo:IAO_0000115>A series of sea caves on the Catlins Coast in New Zealand.</obo:IAO_0000115>
        <oboInOwl:hasOBONamespace>GAZ</oboInOwl:hasOBONamespace>
        <oboInOwl:id>GAZ:00147203</oboInOwl:id>
        <rdfs:label>Cathedral Caves</rdfs:label>
    </owl:NamedIndividual>
    


    <!-- http://purl.obolibrary.org/obo/GAZ_00147204 -->

    <owl:NamedIndividual rdf:about="http://purl.obolibrary.org/obo/GAZ_00147204">
        <rdf:type rdf:resource="http://purl.obolibrary.org/obo/ENVO_00000305"/>
        <obo:RO_0001025 rdf:resource="http://purl.obolibrary.org/obo/GAZ_00004778"/>
        <obo:IAO_0000115>A headland located on the West Coast of New Zealand&apos;s South Island.</obo:IAO_0000115>
        <oboInOwl:hasOBONamespace>GAZ</oboInOwl:hasOBONamespace>
        <oboInOwl:id>GAZ:00147204</oboInOwl:id>
        <rdfs:label>Knight&apos;s Point</rdfs:label>
    </owl:NamedIndividual>
    


    <!-- http://purl.obolibrary.org/obo/GAZ_00153915 -->

    <owl:NamedIndividual rdf:about="http://purl.obolibrary.org/obo/GAZ_00153915">
        <obo:RO_0001025 rdf:resource="http://purl.obolibrary.org/obo/GAZ_00008565"/>
        <obo:IAO_0000115>A topogeneous mire, located three km north of Plimmerton and 20 km north-northeast of Wellington City, New Zealand.</obo:IAO_0000115>
        <oboInOwl:hasOBONamespace>GAZ</oboInOwl:hasOBONamespace>
        <oboInOwl:id>GAZ:00153915</oboInOwl:id>
        <rdfs:label>Taupo Swamp</rdfs:label>
    </owl:NamedIndividual>
    


    <!-- http://purl.obolibrary.org/obo/GAZ_00246620 -->

    <owl:NamedIndividual rdf:about="http://purl.obolibrary.org/obo/GAZ_00246620">
        <obo:RO_0001025 rdf:resource="http://purl.obolibrary.org/obo/GAZ_02000337"/>
        <obo:IAO_0000115>An enclosed brackish lagoon with a small area of salt marsh in the centre of a raised coral atoll.</obo:IAO_0000115>
        <oboInOwl:hasOBONamespace>GAZ</oboInOwl:hasOBONamespace>
        <oboInOwl:id>GAZ:00246620</oboInOwl:id>
        <rdfs:label>Lake Namo</rdfs:label>
    </owl:NamedIndividual>
    


    <!-- http://purl.obolibrary.org/obo/GAZ_00259973 -->

    <owl:NamedIndividual rdf:about="http://purl.obolibrary.org/obo/GAZ_00259973">
        <obo:RO_0001025 rdf:resource="http://purl.obolibrary.org/obo/GAZ_00009561"/>
        <obo:IAO_0000115>An area of reef flat, almost exposed at low tide, with deposits of sand and coral limestone, scattered coral heads and boulders of sedimentary rock.</obo:IAO_0000115>
        <oboInOwl:hasOBONamespace>GAZ</oboInOwl:hasOBONamespace>
        <oboInOwl:id>GAZ:00259973</oboInOwl:id>
        <rdfs:label>Teahagaloa</rdfs:label>
    </owl:NamedIndividual>
    


    <!-- http://purl.obolibrary.org/obo/GAZ_00260233 -->

    <owl:NamedIndividual rdf:about="http://purl.obolibrary.org/obo/GAZ_00260233">
        <obo:RO_0001025 rdf:resource="http://purl.obolibrary.org/obo/GAZ_00009560"/>
        <obo:IAO_0000115>A protected area. Includes a small area along the northern part of the atoll, no land area included. Established 1998.</obo:IAO_0000115>
        <oboInOwl:hasOBONamespace>GAZ</oboInOwl:hasOBONamespace>
        <oboInOwl:id>GAZ:00260233</oboInOwl:id>
        <rdfs:label>Nukunonu Marine Conservation Area</rdfs:label>
    </owl:NamedIndividual>
    


    <!-- http://purl.obolibrary.org/obo/GAZ_00260234 -->

    <owl:NamedIndividual rdf:about="http://purl.obolibrary.org/obo/GAZ_00260234">
        <obo:RO_0001025 rdf:resource="http://purl.obolibrary.org/obo/GAZ_00009562"/>
        <obo:IAO_0000115>A protected area. Includes lagoon area surrounding Fenualoa motu &amp; Atafu village in the north-western corner of the atoll Established 1995.</obo:IAO_0000115>
        <oboInOwl:hasOBONamespace>GAZ</oboInOwl:hasOBONamespace>
        <oboInOwl:id>GAZ:00260234</oboInOwl:id>
        <rdfs:label>Atafu Marine Conservation Area</rdfs:label>
    </owl:NamedIndividual>
    


    <!-- http://purl.obolibrary.org/obo/GAZ_00260235 -->

    <owl:NamedIndividual rdf:about="http://purl.obolibrary.org/obo/GAZ_00260235">
        <obo:RO_0001025 rdf:resource="http://purl.obolibrary.org/obo/GAZ_00009561"/>
        <obo:IAO_0000115>A protected area. Includes the southern corner of the lagoon including the southern motu of Fenualoa and the outside lagoon surrounding the motu. Established 1992.</obo:IAO_0000115>
        <oboInOwl:hasOBONamespace>GAZ</oboInOwl:hasOBONamespace>
        <oboInOwl:id>GAZ:00260235</oboInOwl:id>
        <rdfs:label>Fakaofo Conservation Area</rdfs:label>
    </owl:NamedIndividual>
    


    <!-- http://purl.obolibrary.org/obo/GAZ_02000337 -->

    <owl:NamedIndividual rdf:about="http://purl.obolibrary.org/obo/GAZ_02000337">
        <obo:RO_0001025 rdf:resource="http://purl.obolibrary.org/obo/GAZ_00006949"/>
        <obo:IAO_0000115>An atoll in the Tokelau chain, the most northwesterly island administered by American Samoa. Culturally a part of the Tokelau Islands, politically it is an unorganized territory of the United States of America.</obo:IAO_0000115>
        <oboInOwl:hasOBONamespace>GAZ</oboInOwl:hasOBONamespace>
        <oboInOwl:id>GAZ:02000337</oboInOwl:id>
        <rdfs:label>Swain&apos;s Island</rdfs:label>
    </owl:NamedIndividual>
    


    <!-- http://purl.obolibrary.org/obo/GAZ_22224487 -->

    <owl:NamedIndividual rdf:about="http://purl.obolibrary.org/obo/GAZ_22224487">
        <obo:RO_0001025 rdf:resource="http://purl.obolibrary.org/obo/GAZ_00029928"/>
    </owl:NamedIndividual>
    


    <!-- 
    ///////////////////////////////////////////////////////////////////////////////////////
    //
    // Annotations
    //
    ///////////////////////////////////////////////////////////////////////////////////////
     -->

    <rdf:Description rdf:about="http://purl.obolibrary.org/obo/GAZ_00004759">
        <rdfs:label>Region (New Zealand)</rdfs:label>
        <oboInOwl:id>GAZ:00004759</oboInOwl:id>
        <oboInOwl:hasOBONamespace>GAZ</oboInOwl:hasOBONamespace>
    </rdf:Description>
    <rdf:Description rdf:about="http://purl.obolibrary.org/obo/GAZ_00004760">
        <rdfs:label>Auckland Region</rdfs:label>
        <oboInOwl:hasOBONamespace>GAZ</oboInOwl:hasOBONamespace>
        <oboInOwl:id>GAZ:00004760</oboInOwl:id>
    </rdf:Description>
    <rdf:Description rdf:about="http://purl.obolibrary.org/obo/GAZ_00004762">
        <oboInOwl:hasOBONamespace>GAZ</oboInOwl:hasOBONamespace>
        <rdfs:label>populated place, New Zealand</rdfs:label>
        <oboInOwl:id>GAZ:00004762</oboInOwl:id>
    </rdf:Description>
    <rdf:Description rdf:about="http://purl.obolibrary.org/obo/GAZ_00004767">
        <obo:IAO_0000115>A region of New Zealand in the south of the South Island.</obo:IAO_0000115>
        <oboInOwl:id>GAZ:00004767</oboInOwl:id>
        <rdfs:label>Otago Region</rdfs:label>
        <oboInOwl:hasOBONamespace>GAZ</oboInOwl:hasOBONamespace>
    </rdf:Description>
    <rdf:Description rdf:about="http://purl.obolibrary.org/obo/GAZ_00004768">
        <rdfs:label>Dunedin City</rdfs:label>
        <oboInOwl:id>GAZ:00004768</oboInOwl:id>
        <oboInOwl:hasOBONamespace>GAZ</oboInOwl:hasOBONamespace>
    </rdf:Description>
    <rdf:Description rdf:about="http://purl.obolibrary.org/obo/GAZ_00004770">
        <rdfs:label>Palmerston</rdfs:label>
        <oboInOwl:hasOBONamespace>GAZ</oboInOwl:hasOBONamespace>
        <oboInOwl:id>GAZ:00004770</oboInOwl:id>
    </rdf:Description>
    <rdf:Description rdf:about="http://purl.obolibrary.org/obo/GAZ_00004772">
        <oboInOwl:id>GAZ:00004772</oboInOwl:id>
        <oboInOwl:hasOBONamespace>GAZ</oboInOwl:hasOBONamespace>
        <rdfs:label>Manawatu-Wanganui Region</rdfs:label>
    </rdf:Description>
    <rdf:Description rdf:about="http://purl.obolibrary.org/obo/GAZ_00004773">
        <oboInOwl:hasOBONamespace>GAZ</oboInOwl:hasOBONamespace>
        <rdfs:label>Palmerston North City</rdfs:label>
        <oboInOwl:id>GAZ:00004773</oboInOwl:id>
    </rdf:Description>
    <rdf:Description rdf:about="http://purl.obolibrary.org/obo/GAZ_00004777">
        <oboInOwl:id>GAZ:00004777</oboInOwl:id>
        <oboInOwl:hasOBONamespace>GAZ</oboInOwl:hasOBONamespace>
        <rdfs:label>West Coast Region</rdfs:label>
        <obo:IAO_0000115>An administrative region of New Zealand, located on the west coast of the South Island. The West Coast region reaches from Kahurangi Point in the north to Awarua Point in the south, a distance of 600 km. To the west is the Tasman Sea.</obo:IAO_0000115>
    </rdf:Description>
    <rdf:Description rdf:about="http://purl.obolibrary.org/obo/GAZ_00004781">
        <oboInOwl:hasOBONamespace>GAZ</oboInOwl:hasOBONamespace>
        <rdfs:label>Waikato Region</rdfs:label>
        <oboInOwl:id>GAZ:00004781</oboInOwl:id>
    </rdf:Description>
    <rdf:Description rdf:about="http://purl.obolibrary.org/obo/GAZ_00007723">
        <oboInOwl:id>GAZ:00007723</oboInOwl:id>
        <oboInOwl:hasOBONamespace>GAZ</oboInOwl:hasOBONamespace>
        <rdfs:label>Bay of Plenty Region</rdfs:label>
    </rdf:Description>
    <rdf:Description rdf:about="http://purl.obolibrary.org/obo/GAZ_00007724">
        <oboInOwl:id>GAZ:00007724</oboInOwl:id>
        <oboInOwl:hasOBONamespace>GAZ</oboInOwl:hasOBONamespace>
        <rdfs:label>Rotorua</rdfs:label>
    </rdf:Description>
    <rdf:Description rdf:about="http://purl.obolibrary.org/obo/GAZ_00008561">
        <oboInOwl:id>GAZ:00008561</oboInOwl:id>
        <rdfs:label>Hamilton City</rdfs:label>
        <oboInOwl:hasOBONamespace>GAZ</oboInOwl:hasOBONamespace>
    </rdf:Description>
    <rdf:Description rdf:about="http://purl.obolibrary.org/obo/GAZ_00008562">
        <rdfs:label>Canterbury Region</rdfs:label>
        <oboInOwl:id>GAZ:00008562</oboInOwl:id>
        <obo:IAO_0000115>A region of New Zealand that mainly composed of the Canterbury Plains and the surrounding mountains. Its main city, Christchurch. The region is bounded in the north by the Conway River and to the west by the Southern Alps. The southern boundary is the Waitaki River.</obo:IAO_0000115>
        <oboInOwl:hasOBONamespace>GAZ</oboInOwl:hasOBONamespace>
    </rdf:Description>
    <rdf:Description rdf:about="http://purl.obolibrary.org/obo/GAZ_00008564">
        <oboInOwl:hasOBONamespace>GAZ</oboInOwl:hasOBONamespace>
        <oboInOwl:id>GAZ:00008564</oboInOwl:id>
        <rdfs:label>Taranaki Region</rdfs:label>
        <obo:IAO_0000115>A region in the west of New Zealand&apos;s North Island and is the 10th largest region of New Zealand by population.</obo:IAO_0000115>
    </rdf:Description>
    <rdf:Description rdf:about="http://purl.obolibrary.org/obo/GAZ_00008565">
        <obo:IAO_0000115>A region occupies the southern tip of the North Island, bounded to the west, south, and east by water. To the west lies the Tasman Sea and to the east the Pacific Ocean. At the southern end of the island these two bodies of water are joined by the narrow and turbulent Cook Strait, which is only 28 km wide at its narrowest point, between Cape Terawhiti and Perano Head in the Marlborough Sounds.</obo:IAO_0000115>
        <oboInOwl:hasOBONamespace>GAZ</oboInOwl:hasOBONamespace>
        <rdfs:label>Wellington Region</rdfs:label>
        <oboInOwl:id>GAZ:00008565</oboInOwl:id>
    </rdf:Description>
    <rdf:Description rdf:about="http://purl.obolibrary.org/obo/GAZ_00008568">
        <oboInOwl:hasOBONamespace>GAZ</oboInOwl:hasOBONamespace>
        <oboInOwl:id>GAZ:00008568</oboInOwl:id>
        <obo:IAO_0000115>One of the regions of New Zealand, located in the northeast of the South Island. Marlborough is a unitary authority, both a region and a district, and its council is located at Blenheim.</obo:IAO_0000115>
        <rdfs:label>Marlborough Region</rdfs:label>
    </rdf:Description>
    <rdf:Description rdf:about="http://purl.obolibrary.org/obo/GAZ_00008569">
        <rdfs:label>Northland Region</rdfs:label>
        <oboInOwl:hasOBONamespace>GAZ</oboInOwl:hasOBONamespace>
        <oboInOwl:id>GAZ:00008569</oboInOwl:id>
    </rdf:Description>
    <rdf:Description rdf:about="http://purl.obolibrary.org/obo/GAZ_00008570">
        <oboInOwl:id>GAZ:00008570</oboInOwl:id>
        <oboInOwl:hasOBONamespace>GAZ</oboInOwl:hasOBONamespace>
        <rdfs:label>Whangarei</rdfs:label>
    </rdf:Description>
    <rdf:Description rdf:about="http://purl.obolibrary.org/obo/GAZ_00008571">
        <rdfs:label>Whangarei Harbour</rdfs:label>
        <oboInOwl:id>GAZ:00008571</oboInOwl:id>
        <oboInOwl:hasOBONamespace>GAZ</oboInOwl:hasOBONamespace>
        <obo:IAO_0000115>A large natural harbor whose entrance on the E side of North Auckland Peninsula is between Marsden Point and Bream Head.</obo:IAO_0000115>
    </rdf:Description>
    <rdf:Description rdf:about="http://purl.obolibrary.org/obo/GAZ_00008572">
        <obo:IAO_0000115>The southermost region of New Zealand.</obo:IAO_0000115>
        <oboInOwl:id>GAZ:00008572</oboInOwl:id>
        <oboInOwl:hasOBONamespace>GAZ</oboInOwl:hasOBONamespace>
        <rdfs:label>Southland Region</rdfs:label>
    </rdf:Description>
    <rdf:Description rdf:about="http://purl.obolibrary.org/obo/GAZ_00009534">
        <oboInOwl:id>GAZ:00009534</oboInOwl:id>
        <oboInOwl:hasOBONamespace>GAZ</oboInOwl:hasOBONamespace>
        <rdfs:label>Auckland City</rdfs:label>
    </rdf:Description>
    <rdf:Description rdf:about="http://purl.obolibrary.org/obo/GAZ_00009760">
        <oboInOwl:id>GAZ:00009760</oboInOwl:id>
        <oboInOwl:hasOBONamespace>GAZ</oboInOwl:hasOBONamespace>
        <rdfs:label>Wellington City</rdfs:label>
    </rdf:Description>
    <rdf:Description rdf:about="http://purl.obolibrary.org/obo/GAZ_00009762">
        <oboInOwl:id>GAZ:00009762</oboInOwl:id>
        <oboInOwl:hasOBONamespace>GAZ</oboInOwl:hasOBONamespace>
        <rdfs:label>Upper Hutt City</rdfs:label>
    </rdf:Description>
    <rdf:Description rdf:about="http://purl.obolibrary.org/obo/GAZ_00009763">
        <rdfs:label>Lower Hutt City</rdfs:label>
        <oboInOwl:hasOBONamespace>GAZ</oboInOwl:hasOBONamespace>
        <oboInOwl:id>GAZ:00009763</oboInOwl:id>
    </rdf:Description>
    <rdf:Description rdf:about="http://purl.obolibrary.org/obo/GAZ_00009776">
        <oboInOwl:hasOBONamespace>GAZ</oboInOwl:hasOBONamespace>
        <obo:IAO_0000115>A city located on the South Taranaki Bight, close to the mouth of the Whanganui River. It is 200 km north of Wellington and 75 km northwest of Palmerston North, at the junction of State Highways 3 and 4. Most of the town lies on the NW bank of the river, although some suburbs are located on the opposite side of the river.</obo:IAO_0000115>
        <oboInOwl:id>GAZ:00009776</oboInOwl:id>
        <rdfs:label>Wanganui City</rdfs:label>
    </rdf:Description>
    <rdf:Description rdf:about="http://purl.obolibrary.org/obo/GAZ_00010240">
        <oboInOwl:hasOBONamespace>GAZ</oboInOwl:hasOBONamespace>
        <rdfs:label>Tauranga City</rdfs:label>
        <oboInOwl:id>GAZ:00010240</oboInOwl:id>
    </rdf:Description>
    <rdf:Description rdf:about="http://purl.obolibrary.org/obo/GAZ_00010241">
        <oboInOwl:hasOBONamespace>GAZ</oboInOwl:hasOBONamespace>
        <rdfs:label>Whakatane</rdfs:label>
        <oboInOwl:id>GAZ:00010241</oboInOwl:id>
    </rdf:Description>
    <rdf:Description rdf:about="http://purl.obolibrary.org/obo/GAZ_00010245">
        <rdfs:label>Ashburton</rdfs:label>
        <oboInOwl:id>GAZ:00010245</oboInOwl:id>
        <oboInOwl:hasOBONamespace>GAZ</oboInOwl:hasOBONamespace>
    </rdf:Description>
    <rdf:Description rdf:about="http://purl.obolibrary.org/obo/GAZ_00010246">
        <oboInOwl:id>GAZ:00010246</oboInOwl:id>
        <rdfs:label>Christchurch City</rdfs:label>
        <oboInOwl:hasOBONamespace>GAZ</oboInOwl:hasOBONamespace>
    </rdf:Description>
    <rdf:Description rdf:about="http://purl.obolibrary.org/obo/GAZ_00010247">
        <rdfs:label>Timaru</rdfs:label>
        <oboInOwl:id>GAZ:00010247</oboInOwl:id>
        <oboInOwl:hasOBONamespace>GAZ</oboInOwl:hasOBONamespace>
    </rdf:Description>
    <rdf:Description rdf:about="http://purl.obolibrary.org/obo/GAZ_00010250">
        <oboInOwl:hasOBONamespace>GAZ</oboInOwl:hasOBONamespace>
        <rdfs:label>Blenheim</rdfs:label>
        <oboInOwl:id>GAZ:00010250</oboInOwl:id>
    </rdf:Description>
    <rdf:Description rdf:about="http://purl.obolibrary.org/obo/GAZ_00010251">
        <oboInOwl:hasOBONamespace>GAZ</oboInOwl:hasOBONamespace>
        <obo:IAO_0000115>A city that lies at the shore of Tasman Bay, at the northern end of the South Island, and is the administrative centre of the Nelson region.</obo:IAO_0000115>
        <rdfs:label>Nelson City</rdfs:label>
        <oboInOwl:id>GAZ:00010251</oboInOwl:id>
    </rdf:Description>
    <rdf:Description rdf:about="http://purl.obolibrary.org/obo/GAZ_00010254">
        <rdfs:label>Invercargill City</rdfs:label>
        <oboInOwl:id>GAZ:00010254</oboInOwl:id>
        <oboInOwl:hasOBONamespace>GAZ</oboInOwl:hasOBONamespace>
    </rdf:Description>
    <rdf:Description rdf:about="http://purl.obolibrary.org/obo/GAZ_00010256">
        <obo:IAO_0000115>A region of New Zealand situated on the east coast of the North Island.</obo:IAO_0000115>
        <oboInOwl:id>GAZ:00010256</oboInOwl:id>
        <oboInOwl:hasOBONamespace>GAZ</oboInOwl:hasOBONamespace>
        <rdfs:label>Hawke&apos;s Bay Region</rdfs:label>
    </rdf:Description>
    <rdf:Description rdf:about="http://purl.obolibrary.org/obo/GAZ_00010257">
        <rdfs:label>Dannevirke</rdfs:label>
        <oboInOwl:id>GAZ:00010257</oboInOwl:id>
        <oboInOwl:hasOBONamespace>GAZ</oboInOwl:hasOBONamespace>
    </rdf:Description>
    <rdf:Description rdf:about="http://purl.obolibrary.org/obo/GAZ_00146180">
        <obo:IAO_0000115>A populated place. A town in the Far North District of New Zealand, about 260 km from Auckland.</obo:IAO_0000115>
        <oboInOwl:id>GAZ:00146180</oboInOwl:id>
        <rdfs:label>Kaikohe</rdfs:label>
        <oboInOwl:hasOBONamespace>GAZ</oboInOwl:hasOBONamespace>
    </rdf:Description>
    <rdf:Description rdf:about="http://purl.obolibrary.org/obo/GAZ_00146181">
        <rdfs:label>Ngawha Springs</rdfs:label>
        <obo:IAO_0000115>A small settlement approximately 5 km east of the town of Kaikohe, Northland in New Zealand.</obo:IAO_0000115>
        <oboInOwl:hasOBONamespace>GAZ</oboInOwl:hasOBONamespace>
        <oboInOwl:id>GAZ:00146181</oboInOwl:id>
    </rdf:Description>
    <rdf:Description rdf:about="http://purl.obolibrary.org/obo/GAZ_22224487">
        <oboInOwl:id>GAZ:22224487</oboInOwl:id>
        <rdfs:label>Waitangi</rdfs:label>
        <obo:IAO_0000115>A populated place. A township located in the Bay of Islands on the North Island of New Zealand.</obo:IAO_0000115>
        <oboInOwl:hasOBONamespace>GAZ</oboInOwl:hasOBONamespace>
    </rdf:Description>
</rdf:RDF>



<!-- Generated by the OWL API (version 4.5.6) https://github.com/owlcs/owlapi -->

