<?xml version="1.0"?>
<rdf:RDF xmlns="http://purl.obolibrary.org/obo/gaz/subsets/countries/Nicaragua.owl#"
     xml:base="http://purl.obolibrary.org/obo/gaz/subsets/countries/Nicaragua.owl"
     xmlns:obo="http://purl.obolibrary.org/obo/"
     xmlns:owl="http://www.w3.org/2002/07/owl#"
     xmlns:rdf="http://www.w3.org/1999/02/22-rdf-syntax-ns#"
     xmlns:xml="http://www.w3.org/XML/1998/namespace"
     xmlns:xsd="http://www.w3.org/2001/XMLSchema#"
     xmlns:rdfs="http://www.w3.org/2000/01/rdf-schema#"
     xmlns:oboInOwl="http://www.geneontology.org/formats/oboInOwl#">
    <owl:Ontology rdf:about="http://purl.obolibrary.org/obo/gaz/subsets/countries/Nicaragua.owl">
        <owl:imports rdf:resource="http://purl.obolibrary.org/obo/gaz/imports/envo_import.owl"/>
        <owl:imports rdf:resource="http://purl.obolibrary.org/obo/gaz/imports/ro_import.owl"/>
    </owl:Ontology>
    


    <!-- 
    ///////////////////////////////////////////////////////////////////////////////////////
    //
    // Annotation properties
    //
    ///////////////////////////////////////////////////////////////////////////////////////
     -->

    


    <!-- http://purl.obolibrary.org/obo/IAO_0000115 -->

    <owl:AnnotationProperty rdf:about="http://purl.obolibrary.org/obo/IAO_0000115"/>
    


    <!-- http://www.geneontology.org/formats/oboInOwl#hasOBONamespace -->

    <owl:AnnotationProperty rdf:about="http://www.geneontology.org/formats/oboInOwl#hasOBONamespace"/>
    


    <!-- http://www.geneontology.org/formats/oboInOwl#id -->

    <owl:AnnotationProperty rdf:about="http://www.geneontology.org/formats/oboInOwl#id"/>
    


    <!-- 
    ///////////////////////////////////////////////////////////////////////////////////////
    //
    // Object Properties
    //
    ///////////////////////////////////////////////////////////////////////////////////////
     -->

    


    <!-- http://purl.obolibrary.org/obo/RO_0001025 -->

    <owl:ObjectProperty rdf:about="http://purl.obolibrary.org/obo/RO_0001025"/>
    


    <!-- 
    ///////////////////////////////////////////////////////////////////////////////////////
    //
    // Classes
    //
    ///////////////////////////////////////////////////////////////////////////////////////
     -->

    


    <!-- http://purl.obolibrary.org/obo/ENVO_00000004 -->

    <owl:Class rdf:about="http://purl.obolibrary.org/obo/ENVO_00000004"/>
    


    <!-- http://purl.obolibrary.org/obo/ENVO_00000020 -->

    <owl:Class rdf:about="http://purl.obolibrary.org/obo/ENVO_00000020"/>
    


    <!-- http://purl.obolibrary.org/obo/ENVO_00000095 -->

    <owl:Class rdf:about="http://purl.obolibrary.org/obo/ENVO_00000095"/>
    


    <!-- http://purl.obolibrary.org/obo/ENVO_00000098 -->

    <owl:Class rdf:about="http://purl.obolibrary.org/obo/ENVO_00000098"/>
    


    <!-- http://purl.obolibrary.org/obo/ENVO_00000354 -->

    <owl:Class rdf:about="http://purl.obolibrary.org/obo/ENVO_00000354"/>
    


    <!-- http://purl.obolibrary.org/obo/ENVO_00000856 -->

    <owl:Class rdf:about="http://purl.obolibrary.org/obo/ENVO_00000856"/>
    


    <!-- http://purl.obolibrary.org/obo/GAZ_00000094 -->

    <owl:Class rdf:about="http://purl.obolibrary.org/obo/GAZ_00000094">
        <rdfs:subClassOf rdf:resource="http://purl.obolibrary.org/obo/GAZ_00005221"/>
    </owl:Class>
    


    <!-- http://purl.obolibrary.org/obo/GAZ_00005218 -->

    <owl:Class rdf:about="http://purl.obolibrary.org/obo/GAZ_00005218"/>
    


    <!-- http://purl.obolibrary.org/obo/GAZ_00005219 -->

    <owl:Class rdf:about="http://purl.obolibrary.org/obo/GAZ_00005219">
        <rdfs:subClassOf rdf:resource="http://purl.obolibrary.org/obo/GAZ_00005218"/>
    </owl:Class>
    


    <!-- http://purl.obolibrary.org/obo/GAZ_00005220 -->

    <owl:Class rdf:about="http://purl.obolibrary.org/obo/GAZ_00005220">
        <rdfs:subClassOf rdf:resource="http://purl.obolibrary.org/obo/GAZ_00005221"/>
    </owl:Class>
    


    <!-- http://purl.obolibrary.org/obo/GAZ_00005221 -->

    <owl:Class rdf:about="http://purl.obolibrary.org/obo/GAZ_00005221"/>
    


    <!-- http://purl.obolibrary.org/obo/GAZ_00047242 -->

    <owl:Class rdf:about="http://purl.obolibrary.org/obo/GAZ_00047242"/>
    


    <!-- http://purl.obolibrary.org/obo/GAZ_00047243 -->

    <owl:Class rdf:about="http://purl.obolibrary.org/obo/GAZ_00047243">
        <rdfs:subClassOf rdf:resource="http://purl.obolibrary.org/obo/GAZ_00047242"/>
    </owl:Class>
    


    <!-- http://purl.obolibrary.org/obo/GAZ_00047244 -->

    <owl:Class rdf:about="http://purl.obolibrary.org/obo/GAZ_00047244">
        <rdfs:subClassOf rdf:resource="http://purl.obolibrary.org/obo/GAZ_00047242"/>
    </owl:Class>
    


    <!-- http://purl.obolibrary.org/obo/GAZ_00047261 -->

    <owl:Class rdf:about="http://purl.obolibrary.org/obo/GAZ_00047261">
        <rdfs:subClassOf rdf:resource="http://purl.obolibrary.org/obo/GAZ_00005218"/>
    </owl:Class>
    


    <!-- http://purl.obolibrary.org/obo/GAZ_00056193 -->

    <owl:Class rdf:about="http://purl.obolibrary.org/obo/GAZ_00056193">
        <rdfs:subClassOf rdf:resource="http://purl.obolibrary.org/obo/GAZ_00005218"/>
    </owl:Class>
    


    <!-- http://purl.obolibrary.org/obo/GAZ_00056201 -->

    <owl:Class rdf:about="http://purl.obolibrary.org/obo/GAZ_00056201">
        <rdfs:subClassOf rdf:resource="http://purl.obolibrary.org/obo/GAZ_00005218"/>
    </owl:Class>
    


    <!-- http://purl.obolibrary.org/obo/GAZ_00056204 -->

    <owl:Class rdf:about="http://purl.obolibrary.org/obo/GAZ_00056204">
        <rdfs:subClassOf rdf:resource="http://purl.obolibrary.org/obo/GAZ_00005218"/>
    </owl:Class>
    


    <!-- http://purl.obolibrary.org/obo/GAZ_00056208 -->

    <owl:Class rdf:about="http://purl.obolibrary.org/obo/GAZ_00056208">
        <rdfs:subClassOf rdf:resource="http://purl.obolibrary.org/obo/GAZ_00005218"/>
    </owl:Class>
    


    <!-- http://purl.obolibrary.org/obo/GAZ_00056211 -->

    <owl:Class rdf:about="http://purl.obolibrary.org/obo/GAZ_00056211">
        <rdfs:subClassOf rdf:resource="http://purl.obolibrary.org/obo/GAZ_00005218"/>
    </owl:Class>
    


    <!-- http://purl.obolibrary.org/obo/GAZ_00056214 -->

    <owl:Class rdf:about="http://purl.obolibrary.org/obo/GAZ_00056214">
        <rdfs:subClassOf rdf:resource="http://purl.obolibrary.org/obo/GAZ_00005218"/>
    </owl:Class>
    


    <!-- http://purl.obolibrary.org/obo/GAZ_00062427 -->

    <owl:Class rdf:about="http://purl.obolibrary.org/obo/GAZ_00062427">
        <rdfs:subClassOf rdf:resource="http://purl.obolibrary.org/obo/GAZ_00005218"/>
    </owl:Class>
    


    <!-- http://purl.obolibrary.org/obo/GAZ_00066798 -->

    <owl:Class rdf:about="http://purl.obolibrary.org/obo/GAZ_00066798">
        <rdfs:subClassOf rdf:resource="http://purl.obolibrary.org/obo/GAZ_00005218"/>
    </owl:Class>
    


    <!-- http://purl.obolibrary.org/obo/GAZ_00066799 -->

    <owl:Class rdf:about="http://purl.obolibrary.org/obo/GAZ_00066799">
        <rdfs:subClassOf rdf:resource="http://purl.obolibrary.org/obo/GAZ_00005218"/>
    </owl:Class>
    


    <!-- http://purl.obolibrary.org/obo/GAZ_00066800 -->

    <owl:Class rdf:about="http://purl.obolibrary.org/obo/GAZ_00066800">
        <rdfs:subClassOf rdf:resource="http://purl.obolibrary.org/obo/GAZ_00005218"/>
    </owl:Class>
    


    <!-- http://purl.obolibrary.org/obo/GAZ_00066801 -->

    <owl:Class rdf:about="http://purl.obolibrary.org/obo/GAZ_00066801">
        <rdfs:subClassOf rdf:resource="http://purl.obolibrary.org/obo/GAZ_00005218"/>
    </owl:Class>
    


    <!-- http://purl.obolibrary.org/obo/GAZ_00066802 -->

    <owl:Class rdf:about="http://purl.obolibrary.org/obo/GAZ_00066802">
        <rdfs:subClassOf rdf:resource="http://purl.obolibrary.org/obo/GAZ_00005218"/>
    </owl:Class>
    


    <!-- http://purl.obolibrary.org/obo/GAZ_00066803 -->

    <owl:Class rdf:about="http://purl.obolibrary.org/obo/GAZ_00066803">
        <rdfs:subClassOf rdf:resource="http://purl.obolibrary.org/obo/GAZ_00005218"/>
    </owl:Class>
    


    <!-- 
    ///////////////////////////////////////////////////////////////////////////////////////
    //
    // Individuals
    //
    ///////////////////////////////////////////////////////////////////////////////////////
     -->

    


    <!-- http://purl.obolibrary.org/obo/GAZ_00000094 -->

    <owl:NamedIndividual rdf:about="http://purl.obolibrary.org/obo/GAZ_00000094">
        <obo:RO_0001025 rdf:resource="http://purl.obolibrary.org/obo/GAZ_00066945"/>
    </owl:NamedIndividual>
    


    <!-- http://purl.obolibrary.org/obo/GAZ_00000095 -->

    <owl:NamedIndividual rdf:about="http://purl.obolibrary.org/obo/GAZ_00000095">
        <obo:RO_0001025 rdf:resource="http://purl.obolibrary.org/obo/GAZ_00005219"/>
        <oboInOwl:hasOBONamespace>GAZ</oboInOwl:hasOBONamespace>
        <oboInOwl:id>GAZ:00000095</oboInOwl:id>
        <rdfs:label>Hacienda Apacunca</rdfs:label>
    </owl:NamedIndividual>
    


    <!-- http://purl.obolibrary.org/obo/GAZ_00002978 -->

    <owl:NamedIndividual rdf:about="http://purl.obolibrary.org/obo/GAZ_00002978">
        <obo:IAO_0000115>A republic in Central America. It is also the least densely populated with a demographic similar in size to its smaller neighbors. The country is bordered by Honduras to the north and by Costa Rica to the south. The Pacific Ocean lies to the west of the country, while the Caribbean Sea lies to the east. For administrative purposes it is divided into 15 departments (departamentos) and two self-governing regions (autonomous communities) based on the Spanish model. The departments are then subdivided into 153 municipios (municipalities). The two autonomous regions are Region Autonoma del Atlantico Norte and Region Autonoma del Atlantico Sur, often referred to as RAAN and RAAS, respectively. Until they were granted autonomy in 1985 they formed the single department of Zelaya.</obo:IAO_0000115>
        <oboInOwl:hasOBONamespace>GAZ</oboInOwl:hasOBONamespace>
        <oboInOwl:id>GAZ:00002978</oboInOwl:id>
        <rdfs:label>Nicaragua</rdfs:label>
    </owl:NamedIndividual>
    


    <!-- http://purl.obolibrary.org/obo/GAZ_00005218 -->

    <owl:NamedIndividual rdf:about="http://purl.obolibrary.org/obo/GAZ_00005218">
        <obo:RO_0001025 rdf:resource="http://purl.obolibrary.org/obo/GAZ_00002978"/>
    </owl:NamedIndividual>
    


    <!-- http://purl.obolibrary.org/obo/GAZ_00005219 -->

    <owl:NamedIndividual rdf:about="http://purl.obolibrary.org/obo/GAZ_00005219"/>
    


    <!-- http://purl.obolibrary.org/obo/GAZ_00005220 -->

    <owl:NamedIndividual rdf:about="http://purl.obolibrary.org/obo/GAZ_00005220">
        <rdf:type rdf:resource="http://purl.obolibrary.org/obo/ENVO_00000856"/>
        <obo:RO_0001025 rdf:resource="http://purl.obolibrary.org/obo/GAZ_00012591"/>
    </owl:NamedIndividual>
    


    <!-- http://purl.obolibrary.org/obo/GAZ_00005221 -->

    <owl:NamedIndividual rdf:about="http://purl.obolibrary.org/obo/GAZ_00005221">
        <obo:RO_0001025 rdf:resource="http://purl.obolibrary.org/obo/GAZ_00002978"/>
    </owl:NamedIndividual>
    


    <!-- http://purl.obolibrary.org/obo/GAZ_00012591 -->

    <owl:NamedIndividual rdf:about="http://purl.obolibrary.org/obo/GAZ_00012591">
        <rdf:type rdf:resource="http://purl.obolibrary.org/obo/ENVO_00000856"/>
        <obo:RO_0001025 rdf:resource="http://purl.obolibrary.org/obo/GAZ_00005219"/>
        <obo:IAO_0000115>A municipality in the Chinandega Department of Nicaragua.</obo:IAO_0000115>
        <oboInOwl:hasOBONamespace>GAZ</oboInOwl:hasOBONamespace>
        <oboInOwl:id>GAZ:00012591</oboInOwl:id>
        <rdfs:label>Municipality of Chinandega</rdfs:label>
    </owl:NamedIndividual>
    


    <!-- http://purl.obolibrary.org/obo/GAZ_00047242 -->

    <owl:NamedIndividual rdf:about="http://purl.obolibrary.org/obo/GAZ_00047242">
        <obo:RO_0001025 rdf:resource="http://purl.obolibrary.org/obo/GAZ_00002978"/>
    </owl:NamedIndividual>
    


    <!-- http://purl.obolibrary.org/obo/GAZ_00047243 -->

    <owl:NamedIndividual rdf:about="http://purl.obolibrary.org/obo/GAZ_00047243"/>
    


    <!-- http://purl.obolibrary.org/obo/GAZ_00047244 -->

    <owl:NamedIndividual rdf:about="http://purl.obolibrary.org/obo/GAZ_00047244"/>
    


    <!-- http://purl.obolibrary.org/obo/GAZ_00047245 -->

    <owl:NamedIndividual rdf:about="http://purl.obolibrary.org/obo/GAZ_00047245">
        <obo:RO_0001025 rdf:resource="http://purl.obolibrary.org/obo/GAZ_00047243"/>
        <obo:IAO_0000115>Two islands about 70 km east off the Caribbean coast of Nicaragua, constituting one of 12 municipalities of the Region Autonoma del Atlantico Sur department.</obo:IAO_0000115>
        <oboInOwl:hasOBONamespace>GAZ</oboInOwl:hasOBONamespace>
        <oboInOwl:id>GAZ:00047245</oboInOwl:id>
        <rdfs:label>Corn Islands</rdfs:label>
    </owl:NamedIndividual>
    


    <!-- http://purl.obolibrary.org/obo/GAZ_00047246 -->

    <owl:NamedIndividual rdf:about="http://purl.obolibrary.org/obo/GAZ_00047246">
        <rdf:type rdf:resource="http://purl.obolibrary.org/obo/ENVO_00000856"/>
        <obo:RO_0001025 rdf:resource="http://purl.obolibrary.org/obo/GAZ_00047245"/>
        <obo:IAO_0000115>A municipality in the Corn Islands, Region Autonoma del Atlantico Sur.</obo:IAO_0000115>
        <oboInOwl:hasOBONamespace>GAZ</oboInOwl:hasOBONamespace>
        <oboInOwl:id>GAZ:00047246</oboInOwl:id>
        <rdfs:label>Municipality of Las Islas del Maiz</rdfs:label>
    </owl:NamedIndividual>
    


    <!-- http://purl.obolibrary.org/obo/GAZ_00047247 -->

    <owl:NamedIndividual rdf:about="http://purl.obolibrary.org/obo/GAZ_00047247">
        <obo:RO_0001025 rdf:resource="http://purl.obolibrary.org/obo/GAZ_00047246"/>
        <oboInOwl:hasOBONamespace>GAZ</oboInOwl:hasOBONamespace>
        <oboInOwl:id>GAZ:00047247</oboInOwl:id>
        <rdfs:label>Little Corn Island</rdfs:label>
    </owl:NamedIndividual>
    


    <!-- http://purl.obolibrary.org/obo/GAZ_00047248 -->

    <owl:NamedIndividual rdf:about="http://purl.obolibrary.org/obo/GAZ_00047248">
        <obo:RO_0001025 rdf:resource="http://purl.obolibrary.org/obo/GAZ_00047246"/>
        <oboInOwl:hasOBONamespace>GAZ</oboInOwl:hasOBONamespace>
        <oboInOwl:id>GAZ:00047248</oboInOwl:id>
        <rdfs:label>Big Corn Island</rdfs:label>
    </owl:NamedIndividual>
    


    <!-- http://purl.obolibrary.org/obo/GAZ_00047249 -->

    <owl:NamedIndividual rdf:about="http://purl.obolibrary.org/obo/GAZ_00047249">
        <obo:RO_0001025 rdf:resource="http://purl.obolibrary.org/obo/GAZ_00047244"/>
        <obo:IAO_0000115>An archipelago with an area of 27 km2 located off shore in the North-Eastern Caribbean Coast of Nicaragua, they are part of the RAAN autonomous region. The Miskito Cays are composed of 76 formations that include estuaries, coral reefs, cays, seagrass beds, and islets, of which 12 of the formations are covered with vegetation and consequently form islands which are lined with white sand beaches.</obo:IAO_0000115>
        <oboInOwl:hasOBONamespace>GAZ</oboInOwl:hasOBONamespace>
        <oboInOwl:id>GAZ:00047249</oboInOwl:id>
        <rdfs:label>Cayos Miskitos</rdfs:label>
    </owl:NamedIndividual>
    


    <!-- http://purl.obolibrary.org/obo/GAZ_00047250 -->

    <owl:NamedIndividual rdf:about="http://purl.obolibrary.org/obo/GAZ_00047250">
        <rdf:type rdf:resource="http://purl.obolibrary.org/obo/ENVO_00000098"/>
        <obo:RO_0001025 rdf:resource="http://purl.obolibrary.org/obo/GAZ_00047249"/>
        <obo:IAO_0000115>A cay.</obo:IAO_0000115>
        <oboInOwl:hasOBONamespace>GAZ</oboInOwl:hasOBONamespace>
        <oboInOwl:id>GAZ:00047250</oboInOwl:id>
        <rdfs:label>Cayo Maras</rdfs:label>
    </owl:NamedIndividual>
    


    <!-- http://purl.obolibrary.org/obo/GAZ_00047251 -->

    <owl:NamedIndividual rdf:about="http://purl.obolibrary.org/obo/GAZ_00047251">
        <rdf:type rdf:resource="http://purl.obolibrary.org/obo/ENVO_00000098"/>
        <obo:RO_0001025 rdf:resource="http://purl.obolibrary.org/obo/GAZ_00047249"/>
        <obo:IAO_0000115>A cay.</obo:IAO_0000115>
        <oboInOwl:hasOBONamespace>GAZ</oboInOwl:hasOBONamespace>
        <oboInOwl:id>GAZ:00047251</oboInOwl:id>
        <rdfs:label>Cayo Morrison Denis</rdfs:label>
    </owl:NamedIndividual>
    


    <!-- http://purl.obolibrary.org/obo/GAZ_00047252 -->

    <owl:NamedIndividual rdf:about="http://purl.obolibrary.org/obo/GAZ_00047252">
        <rdf:type rdf:resource="http://purl.obolibrary.org/obo/ENVO_00000098"/>
        <obo:RO_0001025 rdf:resource="http://purl.obolibrary.org/obo/GAZ_00047249"/>
        <obo:IAO_0000115>A cay.</obo:IAO_0000115>
        <oboInOwl:hasOBONamespace>GAZ</oboInOwl:hasOBONamespace>
        <oboInOwl:id>GAZ:00047252</oboInOwl:id>
        <rdfs:label>Cayo Major</rdfs:label>
    </owl:NamedIndividual>
    


    <!-- http://purl.obolibrary.org/obo/GAZ_00047253 -->

    <owl:NamedIndividual rdf:about="http://purl.obolibrary.org/obo/GAZ_00047253">
        <rdf:type rdf:resource="http://purl.obolibrary.org/obo/ENVO_00000098"/>
        <obo:RO_0001025 rdf:resource="http://purl.obolibrary.org/obo/GAZ_00047249"/>
        <obo:IAO_0000115>A cay.</obo:IAO_0000115>
        <oboInOwl:hasOBONamespace>GAZ</oboInOwl:hasOBONamespace>
        <oboInOwl:id>GAZ:00047253</oboInOwl:id>
        <rdfs:label>Cayo Nasa</rdfs:label>
    </owl:NamedIndividual>
    


    <!-- http://purl.obolibrary.org/obo/GAZ_00047254 -->

    <owl:NamedIndividual rdf:about="http://purl.obolibrary.org/obo/GAZ_00047254">
        <obo:RO_0001025 rdf:resource="http://purl.obolibrary.org/obo/GAZ_00047243"/>
        <obo:IAO_0000115>A group of 18 cays located about 35 km from Laguna de Perlas offshore the Caribbean Coast of Nicaragua. They are part of the RAAS autonomous region.</obo:IAO_0000115>
        <oboInOwl:hasOBONamespace>GAZ</oboInOwl:hasOBONamespace>
        <oboInOwl:id>GAZ:00047254</oboInOwl:id>
        <rdfs:label>Cayos Perlas</rdfs:label>
    </owl:NamedIndividual>
    


    <!-- http://purl.obolibrary.org/obo/GAZ_00047255 -->

    <owl:NamedIndividual rdf:about="http://purl.obolibrary.org/obo/GAZ_00047255">
        <obo:RO_0001025 rdf:resource="http://purl.obolibrary.org/obo/GAZ_00267195"/>
        <obo:IAO_0000115>An island in the Bluefields Lagoon on the eastern coast of Nicaragua.</obo:IAO_0000115>
        <oboInOwl:hasOBONamespace>GAZ</oboInOwl:hasOBONamespace>
        <oboInOwl:id>GAZ:00047255</oboInOwl:id>
        <rdfs:label>Rama Cay</rdfs:label>
    </owl:NamedIndividual>
    


    <!-- http://purl.obolibrary.org/obo/GAZ_00047257 -->

    <owl:NamedIndividual rdf:about="http://purl.obolibrary.org/obo/GAZ_00047257">
        <obo:RO_0001025 rdf:resource="http://purl.obolibrary.org/obo/GAZ_00056208"/>
        <obo:IAO_0000115>An island formed by two volcanoes rising from Lake Nicaragua in the Republic of Nicaragua.</obo:IAO_0000115>
        <oboInOwl:hasOBONamespace>GAZ</oboInOwl:hasOBONamespace>
        <oboInOwl:id>GAZ:00047257</oboInOwl:id>
        <rdfs:label>Isla de Ometepe</rdfs:label>
    </owl:NamedIndividual>
    


    <!-- http://purl.obolibrary.org/obo/GAZ_00047258 -->

    <owl:NamedIndividual rdf:about="http://purl.obolibrary.org/obo/GAZ_00047258">
        <obo:RO_0001025 rdf:resource="http://purl.obolibrary.org/obo/GAZ_00267097"/>
        <obo:IAO_0000115>An archipelago of volcanic islands towards the southern end of Lake Nicaragua (also known as Lake Cocibolca) in the Nicaraguan department of Rio San Juan.</obo:IAO_0000115>
        <oboInOwl:hasOBONamespace>GAZ</oboInOwl:hasOBONamespace>
        <oboInOwl:id>GAZ:00047258</oboInOwl:id>
        <rdfs:label>Archipielago de Solentiname</rdfs:label>
    </owl:NamedIndividual>
    


    <!-- http://purl.obolibrary.org/obo/GAZ_00047261 -->

    <owl:NamedIndividual rdf:about="http://purl.obolibrary.org/obo/GAZ_00047261"/>
    


    <!-- http://purl.obolibrary.org/obo/GAZ_00047262 -->

    <owl:NamedIndividual rdf:about="http://purl.obolibrary.org/obo/GAZ_00047262">
        <obo:RO_0001025 rdf:resource="http://purl.obolibrary.org/obo/GAZ_00047258"/>
        <obo:IAO_0000115>An island.</obo:IAO_0000115>
        <oboInOwl:hasOBONamespace>GAZ</oboInOwl:hasOBONamespace>
        <oboInOwl:id>GAZ:00047262</oboInOwl:id>
        <rdfs:label>Isla Mancarron</rdfs:label>
    </owl:NamedIndividual>
    


    <!-- http://purl.obolibrary.org/obo/GAZ_00047263 -->

    <owl:NamedIndividual rdf:about="http://purl.obolibrary.org/obo/GAZ_00047263">
        <obo:RO_0001025 rdf:resource="http://purl.obolibrary.org/obo/GAZ_00047258"/>
        <obo:IAO_0000115>An island.</obo:IAO_0000115>
        <oboInOwl:hasOBONamespace>GAZ</oboInOwl:hasOBONamespace>
        <oboInOwl:id>GAZ:00047263</oboInOwl:id>
        <rdfs:label>Isla La Venada</rdfs:label>
    </owl:NamedIndividual>
    


    <!-- http://purl.obolibrary.org/obo/GAZ_00047264 -->

    <owl:NamedIndividual rdf:about="http://purl.obolibrary.org/obo/GAZ_00047264">
        <obo:RO_0001025 rdf:resource="http://purl.obolibrary.org/obo/GAZ_00047258"/>
        <obo:IAO_0000115>An island.</obo:IAO_0000115>
        <oboInOwl:hasOBONamespace>GAZ</oboInOwl:hasOBONamespace>
        <oboInOwl:id>GAZ:00047264</oboInOwl:id>
        <rdfs:label>Isla Mancarroncito</rdfs:label>
    </owl:NamedIndividual>
    


    <!-- http://purl.obolibrary.org/obo/GAZ_00047265 -->

    <owl:NamedIndividual rdf:about="http://purl.obolibrary.org/obo/GAZ_00047265">
        <obo:RO_0001025 rdf:resource="http://purl.obolibrary.org/obo/GAZ_00047258"/>
        <obo:IAO_0000115>An island.</obo:IAO_0000115>
        <oboInOwl:hasOBONamespace>GAZ</oboInOwl:hasOBONamespace>
        <oboInOwl:id>GAZ:00047265</oboInOwl:id>
        <rdfs:label>Isla San Fernando</rdfs:label>
    </owl:NamedIndividual>
    


    <!-- http://purl.obolibrary.org/obo/GAZ_00047266 -->

    <owl:NamedIndividual rdf:about="http://purl.obolibrary.org/obo/GAZ_00047266">
        <obo:RO_0001025 rdf:resource="http://purl.obolibrary.org/obo/GAZ_00056204"/>
        <obo:IAO_0000115>An archipelago located in Lake Nicaragua, just southeast of the city of Granada in Nicaragua. The islets are a group of over 360 small islands and are scattered about the Asese peninsula. The 365 islets are of volcanic origin they were formed when the Mombacho volcano blew most of its cone into the lake over 20,000 years ago, thereby creating the archipelago.</obo:IAO_0000115>
        <oboInOwl:hasOBONamespace>GAZ</oboInOwl:hasOBONamespace>
        <oboInOwl:id>GAZ:00047266</oboInOwl:id>
        <rdfs:label>Isletas de Granada</rdfs:label>
    </owl:NamedIndividual>
    


    <!-- http://purl.obolibrary.org/obo/GAZ_00047486 -->

    <owl:NamedIndividual rdf:about="http://purl.obolibrary.org/obo/GAZ_00047486">
        <obo:IAO_0000115>A part of the Pacific Ocean, is a gulf in Central America, bordering El Salvador, Honduras and Nicaragua.</obo:IAO_0000115>
        <oboInOwl:hasOBONamespace>GAZ</oboInOwl:hasOBONamespace>
        <oboInOwl:id>GAZ:00047486</oboInOwl:id>
        <rdfs:label>Gulf of Fonseca</rdfs:label>
    </owl:NamedIndividual>
    


    <!-- http://purl.obolibrary.org/obo/GAZ_00047488 -->

    <owl:NamedIndividual rdf:about="http://purl.obolibrary.org/obo/GAZ_00047488">
        <obo:RO_0001025 rdf:resource="http://purl.obolibrary.org/obo/GAZ_00047486"/>
        <obo:IAO_0000115>An island in the in the Gulf of Fonseca, El Salvador.</obo:IAO_0000115>
        <oboInOwl:hasOBONamespace>GAZ</oboInOwl:hasOBONamespace>
        <oboInOwl:id>GAZ:00047488</oboInOwl:id>
        <rdfs:label>Meanguera Island</rdfs:label>
    </owl:NamedIndividual>
    


    <!-- http://purl.obolibrary.org/obo/GAZ_00047489 -->

    <owl:NamedIndividual rdf:about="http://purl.obolibrary.org/obo/GAZ_00047489">
        <obo:RO_0001025 rdf:resource="http://purl.obolibrary.org/obo/GAZ_00047486"/>
        <oboInOwl:hasOBONamespace>GAZ</oboInOwl:hasOBONamespace>
        <oboInOwl:id>GAZ:00047489</oboInOwl:id>
        <rdfs:label>Meanguerita Island</rdfs:label>
    </owl:NamedIndividual>
    


    <!-- http://purl.obolibrary.org/obo/GAZ_00047490 -->

    <owl:NamedIndividual rdf:about="http://purl.obolibrary.org/obo/GAZ_00047490">
        <obo:RO_0001025 rdf:resource="http://purl.obolibrary.org/obo/GAZ_00047486"/>
        <obo:IAO_0000115>A small, 5 km wide island located across a narrow 2 km wide strait south of Isla Zacate Grande in the Gulf of Fonseca. The conical, 783 m high basaltic stratovolcano is the southernmost volcano of Honduras. El Tigre is less dissected than neighboring Zacate Grande volcano on the mainland to the north and is of probable Holocene age. A single satellitic cone, El Vigia, overlooks the village of Amapala on the NW flank.</obo:IAO_0000115>
        <oboInOwl:hasOBONamespace>GAZ</oboInOwl:hasOBONamespace>
        <oboInOwl:id>GAZ:00047490</oboInOwl:id>
        <rdfs:label>El Tigre Island</rdfs:label>
    </owl:NamedIndividual>
    


    <!-- http://purl.obolibrary.org/obo/GAZ_00047491 -->

    <owl:NamedIndividual rdf:about="http://purl.obolibrary.org/obo/GAZ_00047491">
        <obo:RO_0001025 rdf:resource="http://purl.obolibrary.org/obo/GAZ_00047486"/>
        <obo:IAO_0000115>A satellite island off the N coast of El Tigre Island.</obo:IAO_0000115>
        <oboInOwl:hasOBONamespace>GAZ</oboInOwl:hasOBONamespace>
        <oboInOwl:id>GAZ:00047491</oboInOwl:id>
        <rdfs:label>Isla Comandante</rdfs:label>
    </owl:NamedIndividual>
    


    <!-- http://purl.obolibrary.org/obo/GAZ_00047492 -->

    <owl:NamedIndividual rdf:about="http://purl.obolibrary.org/obo/GAZ_00047492">
        <obo:RO_0001025 rdf:resource="http://purl.obolibrary.org/obo/GAZ_00047486"/>
        <obo:IAO_0000115>A stratovolcano that occupies a small, 4 km wide island in the Gulf of Fonseca across a narrow strait from Conchagua volcano. Late-stage eruptions formed a small, sharp-topped cone with a 100-m-wide summit crater at the southern end of the low 505 m high island, and a youthful peninsula also extends from the island&apos;s eastern side. A crescent-shaped crater open to the west is located at the northern end of the island.</obo:IAO_0000115>
        <oboInOwl:hasOBONamespace>GAZ</oboInOwl:hasOBONamespace>
        <oboInOwl:id>GAZ:00047492</oboInOwl:id>
        <rdfs:label>Conchaguita Island</rdfs:label>
    </owl:NamedIndividual>
    


    <!-- http://purl.obolibrary.org/obo/GAZ_00047493 -->

    <owl:NamedIndividual rdf:about="http://purl.obolibrary.org/obo/GAZ_00047493">
        <obo:RO_0001025 rdf:resource="http://purl.obolibrary.org/obo/GAZ_00265029"/>
        <oboInOwl:hasOBONamespace>GAZ</oboInOwl:hasOBONamespace>
        <oboInOwl:id>GAZ:00047493</oboInOwl:id>
        <rdfs:label>Isla Perico</rdfs:label>
    </owl:NamedIndividual>
    


    <!-- http://purl.obolibrary.org/obo/GAZ_00047494 -->

    <owl:NamedIndividual rdf:about="http://purl.obolibrary.org/obo/GAZ_00047494">
        <obo:RO_0001025 rdf:resource="http://purl.obolibrary.org/obo/GAZ_00047486"/>
        <obo:IAO_0000115>An island.</obo:IAO_0000115>
        <oboInOwl:hasOBONamespace>GAZ</oboInOwl:hasOBONamespace>
        <oboInOwl:id>GAZ:00047494</oboInOwl:id>
        <rdfs:label>Isla Martin Perez</rdfs:label>
    </owl:NamedIndividual>
    


    <!-- http://purl.obolibrary.org/obo/GAZ_00056141 -->

    <owl:NamedIndividual rdf:about="http://purl.obolibrary.org/obo/GAZ_00056141">
        <obo:RO_0001025 rdf:resource="http://purl.obolibrary.org/obo/GAZ_00067072"/>
        <obo:IAO_0000115>A lagoon.</obo:IAO_0000115>
        <oboInOwl:hasOBONamespace>GAZ</oboInOwl:hasOBONamespace>
        <oboInOwl:id>GAZ:00056141</oboInOwl:id>
        <rdfs:label>Laguna de Perlas</rdfs:label>
    </owl:NamedIndividual>
    


    <!-- http://purl.obolibrary.org/obo/GAZ_00056183 -->

    <owl:NamedIndividual rdf:about="http://purl.obolibrary.org/obo/GAZ_00056183">
        <obo:RO_0001025 rdf:resource="http://purl.obolibrary.org/obo/GAZ_00047486"/>
        <obo:IAO_0000115>A low 7 x 10 km wide island across a narrow strait from the end of a peninsula surrounded on three sides by the Gulf of Fonseca and Chismuyo bay. Formed by a stratovolcano. At least seven satellitic cones, some of which form small islands offshore, are located from the NE to SE base of the broad 640 m high basaltic stratovolcano. Some of these, including the symmetrical cone of Isla Gueguensi in the tidal flats about 3 km east of the base of Zacate Grande, are of probable Holocene age. In contrast to neighboring Isla El Tigre volcano to the south, Zacate Grande itself is extensively eroded, and deep valleys extend from the summit ridges to the base of the volcano.</obo:IAO_0000115>
        <oboInOwl:hasOBONamespace>GAZ</oboInOwl:hasOBONamespace>
        <oboInOwl:id>GAZ:00056183</oboInOwl:id>
        <rdfs:label>Isla Zacate Grande</rdfs:label>
    </owl:NamedIndividual>
    


    <!-- http://purl.obolibrary.org/obo/GAZ_00056186 -->

    <owl:NamedIndividual rdf:about="http://purl.obolibrary.org/obo/GAZ_00056186">
        <obo:RO_0001025 rdf:resource="http://purl.obolibrary.org/obo/GAZ_00267080"/>
        <obo:IAO_0000115>A low basaltic-to-andesitic composite volcano that is isolated from other eruptive centers in the Nicaraguan volcanic chain. The 872 m high stratovolcano forms a large peninsula extending into the Gulf of Fonseca at the western tip of the country. Cosiguina has a pronounced somma rim on the northern side; a young summit cone of Cosiguina rises 300 m above the northern somma rim and buries the rim on other sides. The younger cone is truncated by a large elliptical prehistorical summit caldera, 2 x 2.4 km in diameter and 500 m deep, with a lake at its bottom. Lava flows predominate in the caldera walls, although lahar and pyroclastic-flow deposits surround the volcano.</obo:IAO_0000115>
        <oboInOwl:hasOBONamespace>GAZ</oboInOwl:hasOBONamespace>
        <oboInOwl:id>GAZ:00056186</oboInOwl:id>
        <rdfs:label>Cosiguina Volcano</rdfs:label>
    </owl:NamedIndividual>
    


    <!-- http://purl.obolibrary.org/obo/GAZ_00056187 -->

    <owl:NamedIndividual rdf:about="http://purl.obolibrary.org/obo/GAZ_00056187">
        <obo:RO_0001025 rdf:resource="http://purl.obolibrary.org/obo/GAZ_00056186"/>
        <obo:IAO_0000115>A crater lake.</obo:IAO_0000115>
        <oboInOwl:hasOBONamespace>GAZ</oboInOwl:hasOBONamespace>
        <oboInOwl:id>GAZ:00056187</oboInOwl:id>
        <rdfs:label>Laguna Cosiguina</rdfs:label>
    </owl:NamedIndividual>
    


    <!-- http://purl.obolibrary.org/obo/GAZ_00056189 -->

    <owl:NamedIndividual rdf:about="http://purl.obolibrary.org/obo/GAZ_00056189">
        <rdf:type rdf:resource="http://purl.obolibrary.org/obo/ENVO_00000354"/>
        <obo:IAO_0000115>A volcanic complex, overlooking Cerro Negro volcano to the NW, that includes a diverse cluster of cones around the central vent, Las Pilas. A N-S-trending fracture system cutting across 1088 m high Las Pilas (El Hoyo) is marked by numerous well-preserved flank vents, including maars, that are part of a 30 km-long volcanic massif. The Cerro Negro chain of cinder cones is listed separately in this compilation because of its extensive historical eruptions. The lake-filled Asososca maar is located adjacent to the conical 818 m high Cerro Asososca cone on the southern side of the fissure system, south of the axis of the Marrabios Range. Two small maars west of Lake Managua are located at the southern end of the fissure.</obo:IAO_0000115>
        <oboInOwl:hasOBONamespace>GAZ</oboInOwl:hasOBONamespace>
        <oboInOwl:id>GAZ:00056189</oboInOwl:id>
        <rdfs:label>Las Pilas Volcanic Complex</rdfs:label>
    </owl:NamedIndividual>
    


    <!-- http://purl.obolibrary.org/obo/GAZ_00056190 -->

    <owl:NamedIndividual rdf:about="http://purl.obolibrary.org/obo/GAZ_00056190">
        <obo:RO_0001025 rdf:resource="http://purl.obolibrary.org/obo/GAZ_00066982"/>
        <obo:RO_0001025 rdf:resource="http://purl.obolibrary.org/obo/GAZ_00267113"/>
        <obo:IAO_0000115>A stratovolcano that has erupted frequently since the beginning of the Spanish era. The Telica volcano group consists of several interlocking cones and vents with a general NW alignment. Sixteenth-century eruptions were reported at symmetrical Santa Clara volcano at the SW end of the Telica group. However, its eroded and breached crater has been covered by forests throughout historical time, and these eruptions may have originated from Telica, whose upper slopes in contrast are unvegetated. The steep-sided cone of 1061 m high Telica is truncated by a 700-m-wide double crater; the southern crater, the source of recent eruptions, is 120 m deep. El Liston, immediately SE of Telica, has several nested craters. The fumaroles and boiling mudpots of Hervideros de San Jacinto, SE of Telica, form a prominent geothermal area frequented by tourists, and geothermal exploration has occurred nearby.</obo:IAO_0000115>
        <oboInOwl:hasOBONamespace>GAZ</oboInOwl:hasOBONamespace>
        <oboInOwl:id>GAZ:00056190</oboInOwl:id>
        <rdfs:label>Volcan Telica</rdfs:label>
    </owl:NamedIndividual>
    


    <!-- http://purl.obolibrary.org/obo/GAZ_00056191 -->

    <owl:NamedIndividual rdf:about="http://purl.obolibrary.org/obo/GAZ_00056191">
        <obo:RO_0001025 rdf:resource="http://purl.obolibrary.org/obo/GAZ_00056193"/>
        <obo:IAO_0000115>The largest, southernmost, and most recent of a group of four youthful cinder cones constructed along a NNW-SSE-trending line in the central Marrabios Range 5 km NW of Las Pilas volcano. Strombolian-to-subplinian eruptions at Cerro Negro at intervals of a few years to several decades have constructed a roughly 250 m high basaltic cone and an associated lava field that is constrained by topography to extend primarily to the NE and SW. Cone and crater morphology at Cerro Negro have varied significantly during its eruptive history. Although Cerro Negro lies in a relatively unpopulated area, its occasional heavy ashfalls have caused damage to crops and buildings in populated regions of the Nicaraguan depression.</obo:IAO_0000115>
        <oboInOwl:hasOBONamespace>GAZ</oboInOwl:hasOBONamespace>
        <oboInOwl:id>GAZ:00056191</oboInOwl:id>
        <rdfs:label>Cerro Negro Volcano</rdfs:label>
    </owl:NamedIndividual>
    


    <!-- http://purl.obolibrary.org/obo/GAZ_00056192 -->

    <owl:NamedIndividual rdf:about="http://purl.obolibrary.org/obo/GAZ_00056192">
        <obo:IAO_0000115>A volcanic complex, that consists of five principal volcanic edifices, forms the NW end of the Marrabios Range. The symmetrical 1745 m high youngest cone, named San Cristobal is Nicaragua&apos;s highest volcano and is capped by a 500 x 600 m wide crater. El Chonco, with several flank lava domes, is located 4 km to the west of San Cristobal; it and the eroded Moyotepe volcano, 4 km to the NE of San Cristobal, are of Pleistocene age. Volcan Casita, containing an elongated summit crater, lies immediately east of San Cristobal and was the site of a catastrophic landslide and lahar in 1998.</obo:IAO_0000115>
        <oboInOwl:hasOBONamespace>GAZ</oboInOwl:hasOBONamespace>
        <oboInOwl:id>GAZ:00056192</oboInOwl:id>
        <rdfs:label>San Cristobal Volcanic Complex</rdfs:label>
    </owl:NamedIndividual>
    


    <!-- http://purl.obolibrary.org/obo/GAZ_00056193 -->

    <owl:NamedIndividual rdf:about="http://purl.obolibrary.org/obo/GAZ_00056193"/>
    


    <!-- http://purl.obolibrary.org/obo/GAZ_00056194 -->

    <owl:NamedIndividual rdf:about="http://purl.obolibrary.org/obo/GAZ_00056194">
        <obo:RO_0001025 rdf:resource="http://purl.obolibrary.org/obo/GAZ_00056192"/>
        <obo:IAO_0000115>A stratovolcano.</obo:IAO_0000115>
        <oboInOwl:hasOBONamespace>GAZ</oboInOwl:hasOBONamespace>
        <oboInOwl:id>GAZ:00056194</oboInOwl:id>
        <rdfs:label>San Cristobal Volcano</rdfs:label>
    </owl:NamedIndividual>
    


    <!-- http://purl.obolibrary.org/obo/GAZ_00056195 -->

    <owl:NamedIndividual rdf:about="http://purl.obolibrary.org/obo/GAZ_00056195">
        <obo:RO_0001025 rdf:resource="http://purl.obolibrary.org/obo/GAZ_00267113"/>
        <obo:IAO_0000115>A stratovolcano of Holocene age occupies the area between Cerro Negro volcano and the Telica volcanic complex in the central Marrabios Range. The 832 m high volcano, also known as Orota, is truncated by a 1 km wide circular crater whose rim is lowest on the southern side. The latest eruption from Rota produced thick andesitic lava flows from a NE-trending fissure NW of the summit. Two small NNW-SSE-trending lava domes, El Bosque (also known as Lomas San Ignacio del Bosque or Cerro Ojochal) are located on the plain 2 km north of the flank of Rota. They were constructed along the same trend as other eruptive fissures that extend transverse to the Marrabios Range volcanoes. An extensive lava field in this area was erupted from numerous small cones and maars.</obo:IAO_0000115>
        <oboInOwl:hasOBONamespace>GAZ</oboInOwl:hasOBONamespace>
        <oboInOwl:id>GAZ:00056195</oboInOwl:id>
        <rdfs:label>Rota Volcano</rdfs:label>
    </owl:NamedIndividual>
    


    <!-- http://purl.obolibrary.org/obo/GAZ_00056196 -->

    <owl:NamedIndividual rdf:about="http://purl.obolibrary.org/obo/GAZ_00056196">
        <obo:RO_0001025 rdf:resource="http://purl.obolibrary.org/obo/GAZ_00056193"/>
        <obo:IAO_0000115>A young, 1297 m high stratovolcano that rises prominently above the NW shore of Lake Managua, forming one of Nicaragua&apos;s most familiar landmarks. Momotombo began growing about 4500 years ago at the SE end of the Marrabios Range and consists of a somma from an older edifice that is surmounted by a symmetrical younger cone with a 150 x 250 m wide summit crater. Young lava flows from Momotombo have flowed down the NW flank into the 4 km wide Monte Galan caldera. The youthful cone of Momotombito forms a 391 m high island offshore in Lake Managua. Momotombo has a long record of strombolian eruptions, punctuated by occasional larger explosive activity. The latest eruption, in 1905, produced a lava flow that traveled from the summit to the lower NE base. A small black plume was seen above the crater after an 1996-04-10 earthquake, but later observations noted no significant changes in the crater. A major geothermal field is located on the southern flank of the volcano.</obo:IAO_0000115>
        <oboInOwl:hasOBONamespace>GAZ</oboInOwl:hasOBONamespace>
        <oboInOwl:id>GAZ:00056196</oboInOwl:id>
        <rdfs:label>Momotombo Volcano</rdfs:label>
    </owl:NamedIndividual>
    


    <!-- http://purl.obolibrary.org/obo/GAZ_00056197 -->

    <owl:NamedIndividual rdf:about="http://purl.obolibrary.org/obo/GAZ_00056197">
        <obo:RO_0001025 rdf:resource="http://purl.obolibrary.org/obo/GAZ_00066801"/>
        <obo:IAO_0000115>A peninsula in Lake Managua.</obo:IAO_0000115>
        <oboInOwl:hasOBONamespace>GAZ</oboInOwl:hasOBONamespace>
        <oboInOwl:id>GAZ:00056197</oboInOwl:id>
        <rdfs:label>Chiltepe Peninsula</rdfs:label>
    </owl:NamedIndividual>
    


    <!-- http://purl.obolibrary.org/obo/GAZ_00056198 -->

    <owl:NamedIndividual rdf:about="http://purl.obolibrary.org/obo/GAZ_00056198">
        <rdf:type rdf:resource="http://purl.obolibrary.org/obo/ENVO_00000354"/>
        <obo:RO_0001025 rdf:resource="http://purl.obolibrary.org/obo/GAZ_00056197"/>
        <obo:IAO_0000115>A volcanic complex that occupies the broad Chiltepe Peninsula, which extends into south-central Lake Managua. The peninsula is part of the Chiltepe pyroclastic shield volcano, one of three large ignimbrite shields on the Nicaraguan volcanic front. A 2.8 km wide, 400-m-deep, lake-filled caldera whose floor lies near sea level truncates the low Apoyeque volcano, which rises only about 500 m above the lake shore. The caldera was the source of a thick mantle of dacitic pumice that blankets the surrounding area. The 2.5 x 3 km wide lake-filled Xiloa (Jiloa) maar, is located immediately SE of Apoyeque. The Talpetatl lava dome was constructed between Laguna Xiloa and Lake Managua. Pumiceous pyroclastic flows from Laguna Xiloa were erupted about 6100 years ago and overlie deposits of comparable age from the Masaya plinian eruption.</obo:IAO_0000115>
        <oboInOwl:hasOBONamespace>GAZ</oboInOwl:hasOBONamespace>
        <oboInOwl:id>GAZ:00056198</oboInOwl:id>
        <rdfs:label>Apoyeque Volcanic Complex</rdfs:label>
    </owl:NamedIndividual>
    


    <!-- http://purl.obolibrary.org/obo/GAZ_00056199 -->

    <owl:NamedIndividual rdf:about="http://purl.obolibrary.org/obo/GAZ_00056199">
        <obo:RO_0001025 rdf:resource="http://purl.obolibrary.org/obo/GAZ_00056198"/>
        <obo:IAO_0000115>A lake-filled maar located immediately SE of Apoyeque Volcano.</obo:IAO_0000115>
        <oboInOwl:hasOBONamespace>GAZ</oboInOwl:hasOBONamespace>
        <oboInOwl:id>GAZ:00056199</oboInOwl:id>
        <rdfs:label>Laguna Xiloa</rdfs:label>
    </owl:NamedIndividual>
    


    <!-- http://purl.obolibrary.org/obo/GAZ_00056200 -->

    <owl:NamedIndividual rdf:about="http://purl.obolibrary.org/obo/GAZ_00056200">
        <obo:RO_0001025 rdf:resource="http://purl.obolibrary.org/obo/GAZ_00066801"/>
        <obo:IAO_0000115>An alignment, located near the western margin of the Nicaraguan graben, cuts through the western part of Nicaragua&apos;s capital city, Managua. This alignment, which has erupted tholeiitic basaltic rocks similar to those from mid-ocean ridges, marks the right-lateral offset of the Nicaraguan volcanic chain. A series of pit craters and fissure vents extends into Lake Managua and is continuous with the volcanic vents on the Chiltepe peninsula. An area of maars and tuff cones perpendicular to the N-S trend of the lineament forms the scalloped shoreline of Lake Managua. Laguna Tiscapa crater is located several km to the east near the central part of the city of Managua. The elongated Nejapa and Ticoma pit craters are surrounded by small basaltic cinder cones and tuff cones. The Nejapa-Miraflores alignment has been the site of about 40 eruptions during the past 30,000 years, the most recent of which (from Cerro Motastepe) occurred less than 2500 years ago.</obo:IAO_0000115>
        <oboInOwl:hasOBONamespace>GAZ</oboInOwl:hasOBONamespace>
        <oboInOwl:id>GAZ:00056200</oboInOwl:id>
        <rdfs:label>Nejapa-Miraflores Fissure Vents</rdfs:label>
    </owl:NamedIndividual>
    


    <!-- http://purl.obolibrary.org/obo/GAZ_00056201 -->

    <owl:NamedIndividual rdf:about="http://purl.obolibrary.org/obo/GAZ_00056201"/>
    


    <!-- http://purl.obolibrary.org/obo/GAZ_00056202 -->

    <owl:NamedIndividual rdf:about="http://purl.obolibrary.org/obo/GAZ_00056202">
        <rdf:type rdf:resource="http://purl.obolibrary.org/obo/ENVO_00000095"/>
        <obo:RO_0001025 rdf:resource="http://purl.obolibrary.org/obo/GAZ_00056201"/>
        <obo:IAO_0000115>A caldera that lies within the massive Pleistocene Las Sierras pyroclastic shield volcano and is a broad, 6 x 11 km basaltic caldera with steep-sided walls up to 300 m high. The caldera is filled on its NW end by more than a dozen vents erupted along a circular, 4 km-diameter fracture system. The twin volcanoes of Nindiri and Masaya, the source of historical eruptions, were constructed at the southern end of the fracture system and contain multiple summit craters, including the currently active Santiago crater. A major basaltic plinian tephra was erupted from Masaya about 6500 years ago. Historical lava flows cover much of the caldera floor and have confined a lake to the far eastern end of the caldera. A lava flow from the 1670 eruption overtopped the north caldera rim.</obo:IAO_0000115>
        <oboInOwl:hasOBONamespace>GAZ</oboInOwl:hasOBONamespace>
        <oboInOwl:id>GAZ:00056202</oboInOwl:id>
        <rdfs:label>Masaya Volcano</rdfs:label>
    </owl:NamedIndividual>
    


    <!-- http://purl.obolibrary.org/obo/GAZ_00056203 -->

    <owl:NamedIndividual rdf:about="http://purl.obolibrary.org/obo/GAZ_00056203">
        <obo:RO_0001025 rdf:resource="http://purl.obolibrary.org/obo/GAZ_00056204"/>
        <obo:IAO_0000115>A semi-arcuate, N-S-trending fissure located between the city of Granada and the eastern rim of Apoyo caldera was the source of the Granada alignment of small cinder cones and craters. The lineament (also known as the La Joya alignment after La Joya explosions craters SW of Granada) cuts across the flanks of Apoyo caldera only 2 km from its rim. However, the Granada alignment is structurally distinct from the caldera and is analogous to the Nejapa-Miraflores alignment north of Masaya volcano. The lineament extends from north of Granada to the northern flanks of Mombacho volcano and is characterized by the eruption of basaltic lavas and tephras compositionally similar to mid-ocean ridge basalts. A series of interconnecting collapse-explosion pits similar to those at Nejapa-Miraflores lies immediately east of the Granada cinder cone alignment. The Granada lineament originated about 12,000 years ago, and the latest eruptions may have occurred as recently as about 2000 years ago.</obo:IAO_0000115>
        <oboInOwl:hasOBONamespace>GAZ</oboInOwl:hasOBONamespace>
        <oboInOwl:id>GAZ:00056203</oboInOwl:id>
        <rdfs:label>Granada Fissure Vents</rdfs:label>
    </owl:NamedIndividual>
    


    <!-- http://purl.obolibrary.org/obo/GAZ_00056204 -->

    <owl:NamedIndividual rdf:about="http://purl.obolibrary.org/obo/GAZ_00056204"/>
    


    <!-- http://purl.obolibrary.org/obo/GAZ_00056206 -->

    <owl:NamedIndividual rdf:about="http://purl.obolibrary.org/obo/GAZ_00056206">
        <obo:IAO_0000115>An andesitic and basaltic stratovolcano on the shores of Lake Nicaragua south of the city of Granada that has undergone edifice collapse on several occasions. Two large horseshoe-shaped craters formed by edifice failure cut the summit on the NE and southern flanks. The NE-flank scarp was the source of a large debris avalanche that produced an arcuate peninsula and a cluster of small islands (Las Isletas) in Lake Nicaragua. Two small, well-preserved cinder cones are located on the volcano&apos;s lower northern flank.</obo:IAO_0000115>
        <oboInOwl:hasOBONamespace>GAZ</oboInOwl:hasOBONamespace>
        <oboInOwl:id>GAZ:00056206</oboInOwl:id>
        <rdfs:label>Mombacho Volcano</rdfs:label>
    </owl:NamedIndividual>
    


    <!-- http://purl.obolibrary.org/obo/GAZ_00056207 -->

    <owl:NamedIndividual rdf:about="http://purl.obolibrary.org/obo/GAZ_00056207">
        <obo:RO_0001025 rdf:resource="http://purl.obolibrary.org/obo/GAZ_00267084"/>
        <obo:IAO_0000115>A small low shield volcano that forms a 7 x 10 km wide island on the western side of Lake Nicaragua just offshore from Mombacho volcano. The island contains some of the most significant archaeological sites in Nicaragua. The small, roughly circular 2 km wide El Llano caldera is located near the center of the island, which is cut by a series of NE-trending faults that continue into Lake Nicaragua. The conical 305 m high Cerro El Llano lava dome occupies the center of the caldera, and other lava domes are found on the southern and NE flanks. Numerous low-rimmed tuff rings and maars, of which Laguna de Zapatera on the NW flank is the best-preserved, are found on the northern and western sides of the densely forested 629 m high island and across a narrow strait on the adjacent mainland.</obo:IAO_0000115>
        <oboInOwl:hasOBONamespace>GAZ</oboInOwl:hasOBONamespace>
        <oboInOwl:id>GAZ:00056207</oboInOwl:id>
        <rdfs:label>Isla de Zapatera</rdfs:label>
    </owl:NamedIndividual>
    


    <!-- http://purl.obolibrary.org/obo/GAZ_00056208 -->

    <owl:NamedIndividual rdf:about="http://purl.obolibrary.org/obo/GAZ_00056208"/>
    


    <!-- http://purl.obolibrary.org/obo/GAZ_00056209 -->

    <owl:NamedIndividual rdf:about="http://purl.obolibrary.org/obo/GAZ_00056209">
        <obo:RO_0001025 rdf:resource="http://purl.obolibrary.org/obo/GAZ_00047257"/>
        <obo:IAO_0000115>A symmetrical basaltic-to-dacitic stratovolcano that forms the NW half of the dumbbell-shaped island of Ometepe in Lake Nicaragua and is connected to neighboring Madera volcano by a narrow isthmus. A steep-walled summit crater is 250 m deep and has a higher western rim. N-S-trending fractures on the flanks of the volcano have produced chains of spatter cones, cinder cones, lava domes, and maars located on the NW, NE, SE, and southern sides extending in some cases down to Lake Nicaragua. Concepcion was constructed above a basement of lake sediments, and the modern cone grew above a largely buried caldera, a small remnant of which forms a break in slope about halfway up the north flank. Frequent explosive eruptions during the past half century have increased the height of the summit significantly above that shown on current topographic maps and have kept the upper part of the volcano unvegetated.</obo:IAO_0000115>
        <oboInOwl:hasOBONamespace>GAZ</oboInOwl:hasOBONamespace>
        <oboInOwl:id>GAZ:00056209</oboInOwl:id>
        <rdfs:label>Volcan Concepcion</rdfs:label>
    </owl:NamedIndividual>
    


    <!-- http://purl.obolibrary.org/obo/GAZ_00056210 -->

    <owl:NamedIndividual rdf:about="http://purl.obolibrary.org/obo/GAZ_00056210">
        <obo:RO_0001025 rdf:resource="http://purl.obolibrary.org/obo/GAZ_00267106"/>
        <obo:IAO_0000115>A roughly conical, 1394 m high stratovolcano that forms the SE end of the dumbbell-shaped Ometepe island in Lake Nicaragua. The basaltic-to-dacitic volcano is cut by numerous faults and grabens, the largest of which is a NW-SE-oriented graben that cuts the summit and has at least 140 m of vertical displacement. The small Laguna de Maderas lake occupies the bottom of the 800-m-wide summit crater, which is located at the western side of the central graben. The SW side of the edifice has been affected by large-scale slumping. Many pyroclastic cones are situated on the lower NE flank down to the level of Lake Nicaragua. The latest period of major growth of Maderas took place more than 3000 years ago. No confirmed historical eruptions are known from the volcano.</obo:IAO_0000115>
        <oboInOwl:hasOBONamespace>GAZ</oboInOwl:hasOBONamespace>
        <oboInOwl:id>GAZ:00056210</oboInOwl:id>
        <rdfs:label>Volcan Maderas</rdfs:label>
    </owl:NamedIndividual>
    


    <!-- http://purl.obolibrary.org/obo/GAZ_00056211 -->

    <owl:NamedIndividual rdf:about="http://purl.obolibrary.org/obo/GAZ_00056211"/>
    


    <!-- http://purl.obolibrary.org/obo/GAZ_00056212 -->

    <owl:NamedIndividual rdf:about="http://purl.obolibrary.org/obo/GAZ_00056212">
        <obo:RO_0001025 rdf:resource="http://purl.obolibrary.org/obo/GAZ_00056211"/>
        <obo:IAO_0000115>Fissure vents that are located in valleys in the northern interior highlands between the town of Esteli and the border with Honduras. McBirney and Williams (1965) considered basaltic flows in this area to be certainly of Quaternary, and possibly of Holocene age. The lava flows near Esteli were faulted and slightly tilted during formation of the Esteli structural basin.</obo:IAO_0000115>
        <oboInOwl:hasOBONamespace>GAZ</oboInOwl:hasOBONamespace>
        <oboInOwl:id>GAZ:00056212</oboInOwl:id>
        <rdfs:label>Esteli Fissure Vents</rdfs:label>
    </owl:NamedIndividual>
    


    <!-- http://purl.obolibrary.org/obo/GAZ_00056213 -->

    <owl:NamedIndividual rdf:about="http://purl.obolibrary.org/obo/GAZ_00056213">
        <obo:RO_0001025 rdf:resource="http://purl.obolibrary.org/obo/GAZ_00066801"/>
        <obo:IAO_0000115>One of several Quaternary volcanoes that lie in the Nicaraguan interior highlands, east of the Nicaraguan depression. The steep-sided stratovolcano was constructed east of the Rio Pacora, NE of Lake Managua at the boundary of the flat-lying Tertiary ignimbrite deposits with the fault-blocks bordering the Nicaraguan depression. A small lava flow extends a short distance beyond the base of the cone through a breach in the SW wall of the well-preserved 1.5 km wide crater. A blocky plug dome occupies the center of the crater.</obo:IAO_0000115>
        <oboInOwl:hasOBONamespace>GAZ</oboInOwl:hasOBONamespace>
        <oboInOwl:id>GAZ:00056213</oboInOwl:id>
        <rdfs:label>Cerro el Ciguatepe</rdfs:label>
    </owl:NamedIndividual>
    


    <!-- http://purl.obolibrary.org/obo/GAZ_00056214 -->

    <owl:NamedIndividual rdf:about="http://purl.obolibrary.org/obo/GAZ_00056214"/>
    


    <!-- http://purl.obolibrary.org/obo/GAZ_00056215 -->

    <owl:NamedIndividual rdf:about="http://purl.obolibrary.org/obo/GAZ_00056215">
        <rdf:type rdf:resource="http://purl.obolibrary.org/obo/ENVO_00000020"/>
        <obo:RO_0001025 rdf:resource="http://purl.obolibrary.org/obo/GAZ_00056214"/>
        <obo:IAO_0000115>A broad, low, basaltic shield volcano is truncated by a 7 km wide, steep-walled caldera. The 650-m-deep caldera is breached by a narrow canyon on the SE side that drains into Lake Nicaragua. Five coalescing andesitic-dacitic lava domes are located in the center of the caldera, and additional domes are present on the outer flanks.</obo:IAO_0000115>
        <oboInOwl:hasOBONamespace>GAZ</oboInOwl:hasOBONamespace>
        <oboInOwl:id>GAZ:00056215</oboInOwl:id>
        <rdfs:label>Volcan Las Lajas</rdfs:label>
    </owl:NamedIndividual>
    


    <!-- http://purl.obolibrary.org/obo/GAZ_00056216 -->

    <owl:NamedIndividual rdf:about="http://purl.obolibrary.org/obo/GAZ_00056216">
        <obo:RO_0001025 rdf:resource="http://purl.obolibrary.org/obo/GAZ_00047243"/>
        <obo:IAO_0000115>A complex of three youthful cinder cones on the jungle-covered Atlantic coastal plain of Nicaragua that were first noted by geologists during an aerial overflight in the 1960s. The three cones, located south of the Rio Curinhuas and west of Pearl Lagoon, each have well-defined, steep-walled craters about 50-60 m across.</obo:IAO_0000115>
        <oboInOwl:hasOBONamespace>GAZ</oboInOwl:hasOBONamespace>
        <oboInOwl:id>GAZ:00056216</oboInOwl:id>
        <rdfs:label>Volcan Azul</rdfs:label>
    </owl:NamedIndividual>
    


    <!-- http://purl.obolibrary.org/obo/GAZ_00062426 -->

    <owl:NamedIndividual rdf:about="http://purl.obolibrary.org/obo/GAZ_00062426">
        <obo:RO_0001025 rdf:resource="http://purl.obolibrary.org/obo/GAZ_00062427"/>
        <obo:IAO_0000115>A reservoir located in the north of Nicaragua. It is created by the dam on the Rio Tuma to the north of Jinotega. The reservoir has an area of 51 km2.</obo:IAO_0000115>
        <oboInOwl:hasOBONamespace>GAZ</oboInOwl:hasOBONamespace>
        <oboInOwl:id>GAZ:00062426</oboInOwl:id>
        <rdfs:label>Lake Apanas</rdfs:label>
    </owl:NamedIndividual>
    


    <!-- http://purl.obolibrary.org/obo/GAZ_00062427 -->

    <owl:NamedIndividual rdf:about="http://purl.obolibrary.org/obo/GAZ_00062427"/>
    


    <!-- http://purl.obolibrary.org/obo/GAZ_00066798 -->

    <owl:NamedIndividual rdf:about="http://purl.obolibrary.org/obo/GAZ_00066798"/>
    


    <!-- http://purl.obolibrary.org/obo/GAZ_00066799 -->

    <owl:NamedIndividual rdf:about="http://purl.obolibrary.org/obo/GAZ_00066799"/>
    


    <!-- http://purl.obolibrary.org/obo/GAZ_00066800 -->

    <owl:NamedIndividual rdf:about="http://purl.obolibrary.org/obo/GAZ_00066800"/>
    


    <!-- http://purl.obolibrary.org/obo/GAZ_00066801 -->

    <owl:NamedIndividual rdf:about="http://purl.obolibrary.org/obo/GAZ_00066801"/>
    


    <!-- http://purl.obolibrary.org/obo/GAZ_00066802 -->

    <owl:NamedIndividual rdf:about="http://purl.obolibrary.org/obo/GAZ_00066802"/>
    


    <!-- http://purl.obolibrary.org/obo/GAZ_00066803 -->

    <owl:NamedIndividual rdf:about="http://purl.obolibrary.org/obo/GAZ_00066803"/>
    


    <!-- http://purl.obolibrary.org/obo/GAZ_00066926 -->

    <owl:NamedIndividual rdf:about="http://purl.obolibrary.org/obo/GAZ_00066926">
        <rdf:type rdf:resource="http://purl.obolibrary.org/obo/ENVO_00000856"/>
        <obo:RO_0001025 rdf:resource="http://purl.obolibrary.org/obo/GAZ_00056214"/>
        <obo:IAO_0000115>A municipality of the Boaco Department of Nicaragua.</obo:IAO_0000115>
        <oboInOwl:hasOBONamespace>GAZ</oboInOwl:hasOBONamespace>
        <oboInOwl:id>GAZ:00066926</oboInOwl:id>
        <rdfs:label>Municipality of San Lorenzo</rdfs:label>
    </owl:NamedIndividual>
    


    <!-- http://purl.obolibrary.org/obo/GAZ_00066927 -->

    <owl:NamedIndividual rdf:about="http://purl.obolibrary.org/obo/GAZ_00066927">
        <rdf:type rdf:resource="http://purl.obolibrary.org/obo/ENVO_00000856"/>
        <obo:RO_0001025 rdf:resource="http://purl.obolibrary.org/obo/GAZ_00056214"/>
        <obo:IAO_0000115>A municipality of the Boaco Department of Nicaragua.</obo:IAO_0000115>
        <oboInOwl:hasOBONamespace>GAZ</oboInOwl:hasOBONamespace>
        <oboInOwl:id>GAZ:00066927</oboInOwl:id>
        <rdfs:label>Municipality of Teustepe</rdfs:label>
    </owl:NamedIndividual>
    


    <!-- http://purl.obolibrary.org/obo/GAZ_00066928 -->

    <owl:NamedIndividual rdf:about="http://purl.obolibrary.org/obo/GAZ_00066928">
        <rdf:type rdf:resource="http://purl.obolibrary.org/obo/ENVO_00000856"/>
        <obo:RO_0001025 rdf:resource="http://purl.obolibrary.org/obo/GAZ_00056214"/>
        <obo:IAO_0000115>A municipality of the Boaco Department of Nicaragua.</obo:IAO_0000115>
        <oboInOwl:hasOBONamespace>GAZ</oboInOwl:hasOBONamespace>
        <oboInOwl:id>GAZ:00066928</oboInOwl:id>
        <rdfs:label>Municipality of Camoapa</rdfs:label>
    </owl:NamedIndividual>
    


    <!-- http://purl.obolibrary.org/obo/GAZ_00066929 -->

    <owl:NamedIndividual rdf:about="http://purl.obolibrary.org/obo/GAZ_00066929">
        <rdf:type rdf:resource="http://purl.obolibrary.org/obo/ENVO_00000856"/>
        <obo:RO_0001025 rdf:resource="http://purl.obolibrary.org/obo/GAZ_00056214"/>
        <obo:IAO_0000115>A municipality of the Boaco Department of Nicaragua.</obo:IAO_0000115>
        <oboInOwl:hasOBONamespace>GAZ</oboInOwl:hasOBONamespace>
        <oboInOwl:id>GAZ:00066929</oboInOwl:id>
        <rdfs:label>Municipality of San Jose de los Remates</rdfs:label>
    </owl:NamedIndividual>
    


    <!-- http://purl.obolibrary.org/obo/GAZ_00066930 -->

    <owl:NamedIndividual rdf:about="http://purl.obolibrary.org/obo/GAZ_00066930">
        <rdf:type rdf:resource="http://purl.obolibrary.org/obo/ENVO_00000856"/>
        <obo:RO_0001025 rdf:resource="http://purl.obolibrary.org/obo/GAZ_00056214"/>
        <obo:IAO_0000115>A municipality of the Boaco Department of Nicaragua.</obo:IAO_0000115>
        <oboInOwl:hasOBONamespace>GAZ</oboInOwl:hasOBONamespace>
        <oboInOwl:id>GAZ:00066930</oboInOwl:id>
        <rdfs:label>Municipality of Boaco</rdfs:label>
    </owl:NamedIndividual>
    


    <!-- http://purl.obolibrary.org/obo/GAZ_00066931 -->

    <owl:NamedIndividual rdf:about="http://purl.obolibrary.org/obo/GAZ_00066931">
        <rdf:type rdf:resource="http://purl.obolibrary.org/obo/ENVO_00000856"/>
        <obo:RO_0001025 rdf:resource="http://purl.obolibrary.org/obo/GAZ_00056214"/>
        <obo:IAO_0000115>A municipality of the Boaco Department of Nicaragua.</obo:IAO_0000115>
        <oboInOwl:hasOBONamespace>GAZ</oboInOwl:hasOBONamespace>
        <oboInOwl:id>GAZ:00066931</oboInOwl:id>
        <rdfs:label>Municipality of Santa Lucia</rdfs:label>
    </owl:NamedIndividual>
    


    <!-- http://purl.obolibrary.org/obo/GAZ_00066932 -->

    <owl:NamedIndividual rdf:about="http://purl.obolibrary.org/obo/GAZ_00066932">
        <rdf:type rdf:resource="http://purl.obolibrary.org/obo/ENVO_00000856"/>
        <obo:RO_0001025 rdf:resource="http://purl.obolibrary.org/obo/GAZ_00066799"/>
        <obo:IAO_0000115>A municipality in the Carazo Department of Nicaragua.</obo:IAO_0000115>
        <oboInOwl:hasOBONamespace>GAZ</oboInOwl:hasOBONamespace>
        <oboInOwl:id>GAZ:00066932</oboInOwl:id>
        <rdfs:label>Municipality of Diriamba</rdfs:label>
    </owl:NamedIndividual>
    


    <!-- http://purl.obolibrary.org/obo/GAZ_00066933 -->

    <owl:NamedIndividual rdf:about="http://purl.obolibrary.org/obo/GAZ_00066933">
        <rdf:type rdf:resource="http://purl.obolibrary.org/obo/ENVO_00000856"/>
        <obo:RO_0001025 rdf:resource="http://purl.obolibrary.org/obo/GAZ_00066799"/>
        <obo:IAO_0000115>A municipality in the Carazo Department of Nicaragua.</obo:IAO_0000115>
        <oboInOwl:hasOBONamespace>GAZ</oboInOwl:hasOBONamespace>
        <oboInOwl:id>GAZ:00066933</oboInOwl:id>
        <rdfs:label>Municipality of Dolores</rdfs:label>
    </owl:NamedIndividual>
    


    <!-- http://purl.obolibrary.org/obo/GAZ_00066934 -->

    <owl:NamedIndividual rdf:about="http://purl.obolibrary.org/obo/GAZ_00066934">
        <rdf:type rdf:resource="http://purl.obolibrary.org/obo/ENVO_00000856"/>
        <obo:RO_0001025 rdf:resource="http://purl.obolibrary.org/obo/GAZ_00066799"/>
        <obo:IAO_0000115>A municipality in the Carazo Department of Nicaragua.</obo:IAO_0000115>
        <oboInOwl:hasOBONamespace>GAZ</oboInOwl:hasOBONamespace>
        <oboInOwl:id>GAZ:00066934</oboInOwl:id>
        <rdfs:label>Municipality of Santa Teresa</rdfs:label>
    </owl:NamedIndividual>
    


    <!-- http://purl.obolibrary.org/obo/GAZ_00066935 -->

    <owl:NamedIndividual rdf:about="http://purl.obolibrary.org/obo/GAZ_00066935">
        <rdf:type rdf:resource="http://purl.obolibrary.org/obo/ENVO_00000856"/>
        <obo:RO_0001025 rdf:resource="http://purl.obolibrary.org/obo/GAZ_00066799"/>
        <obo:IAO_0000115>A municipality in the Carazo Department of Nicaragua.</obo:IAO_0000115>
        <oboInOwl:hasOBONamespace>GAZ</oboInOwl:hasOBONamespace>
        <oboInOwl:id>GAZ:00066935</oboInOwl:id>
        <rdfs:label>Municipality of La Paz de Carazo</rdfs:label>
    </owl:NamedIndividual>
    


    <!-- http://purl.obolibrary.org/obo/GAZ_00066936 -->

    <owl:NamedIndividual rdf:about="http://purl.obolibrary.org/obo/GAZ_00066936">
        <rdf:type rdf:resource="http://purl.obolibrary.org/obo/ENVO_00000856"/>
        <obo:RO_0001025 rdf:resource="http://purl.obolibrary.org/obo/GAZ_00066799"/>
        <obo:IAO_0000115>A municipality in the Carazo Department of Nicaragua.</obo:IAO_0000115>
        <oboInOwl:hasOBONamespace>GAZ</oboInOwl:hasOBONamespace>
        <oboInOwl:id>GAZ:00066936</oboInOwl:id>
        <rdfs:label>Municipality of Jinotepe</rdfs:label>
    </owl:NamedIndividual>
    


    <!-- http://purl.obolibrary.org/obo/GAZ_00066937 -->

    <owl:NamedIndividual rdf:about="http://purl.obolibrary.org/obo/GAZ_00066937">
        <rdf:type rdf:resource="http://purl.obolibrary.org/obo/ENVO_00000856"/>
        <obo:RO_0001025 rdf:resource="http://purl.obolibrary.org/obo/GAZ_00066799"/>
        <obo:IAO_0000115>A municipality in the Carazo Department of Nicaragua.</obo:IAO_0000115>
        <oboInOwl:hasOBONamespace>GAZ</oboInOwl:hasOBONamespace>
        <oboInOwl:id>GAZ:00066937</oboInOwl:id>
        <rdfs:label>Municipality of La Conquista</rdfs:label>
    </owl:NamedIndividual>
    


    <!-- http://purl.obolibrary.org/obo/GAZ_00066938 -->

    <owl:NamedIndividual rdf:about="http://purl.obolibrary.org/obo/GAZ_00066938">
        <rdf:type rdf:resource="http://purl.obolibrary.org/obo/ENVO_00000856"/>
        <obo:RO_0001025 rdf:resource="http://purl.obolibrary.org/obo/GAZ_00066799"/>
        <obo:IAO_0000115>A municipality in the Carazo Department of Nicaragua.</obo:IAO_0000115>
        <oboInOwl:hasOBONamespace>GAZ</oboInOwl:hasOBONamespace>
        <oboInOwl:id>GAZ:00066938</oboInOwl:id>
        <rdfs:label>Municipality of El Rosario</rdfs:label>
    </owl:NamedIndividual>
    


    <!-- http://purl.obolibrary.org/obo/GAZ_00066939 -->

    <owl:NamedIndividual rdf:about="http://purl.obolibrary.org/obo/GAZ_00066939">
        <rdf:type rdf:resource="http://purl.obolibrary.org/obo/ENVO_00000856"/>
        <obo:RO_0001025 rdf:resource="http://purl.obolibrary.org/obo/GAZ_00066799"/>
        <obo:IAO_0000115>A municipality in the Carazo Department of Nicaragua.</obo:IAO_0000115>
        <oboInOwl:hasOBONamespace>GAZ</oboInOwl:hasOBONamespace>
        <oboInOwl:id>GAZ:00066939</oboInOwl:id>
        <rdfs:label>Municipality of San Marcos</rdfs:label>
    </owl:NamedIndividual>
    


    <!-- http://purl.obolibrary.org/obo/GAZ_00066940 -->

    <owl:NamedIndividual rdf:about="http://purl.obolibrary.org/obo/GAZ_00066940">
        <rdf:type rdf:resource="http://purl.obolibrary.org/obo/ENVO_00000856"/>
        <obo:RO_0001025 rdf:resource="http://purl.obolibrary.org/obo/GAZ_00005219"/>
        <obo:IAO_0000115>A municipality in the Chinandega Department of Nicaragua.</obo:IAO_0000115>
        <oboInOwl:hasOBONamespace>GAZ</oboInOwl:hasOBONamespace>
        <oboInOwl:id>GAZ:00066940</oboInOwl:id>
        <rdfs:label>Municipality of San Juan de Cinco Pinos</rdfs:label>
    </owl:NamedIndividual>
    


    <!-- http://purl.obolibrary.org/obo/GAZ_00066941 -->

    <owl:NamedIndividual rdf:about="http://purl.obolibrary.org/obo/GAZ_00066941">
        <rdf:type rdf:resource="http://purl.obolibrary.org/obo/ENVO_00000856"/>
        <obo:RO_0001025 rdf:resource="http://purl.obolibrary.org/obo/GAZ_00005219"/>
        <obo:IAO_0000115>A municipality in the Chinandega Department of Nicaragua.</obo:IAO_0000115>
        <oboInOwl:hasOBONamespace>GAZ</oboInOwl:hasOBONamespace>
        <oboInOwl:id>GAZ:00066941</oboInOwl:id>
        <rdfs:label>Municipality of Villa Nueva</rdfs:label>
    </owl:NamedIndividual>
    


    <!-- http://purl.obolibrary.org/obo/GAZ_00066942 -->

    <owl:NamedIndividual rdf:about="http://purl.obolibrary.org/obo/GAZ_00066942">
        <rdf:type rdf:resource="http://purl.obolibrary.org/obo/ENVO_00000856"/>
        <obo:RO_0001025 rdf:resource="http://purl.obolibrary.org/obo/GAZ_00005219"/>
        <obo:IAO_0000115>A municipality in the Chinandega Department of Nicaragua.</obo:IAO_0000115>
        <oboInOwl:hasOBONamespace>GAZ</oboInOwl:hasOBONamespace>
        <oboInOwl:id>GAZ:00066942</oboInOwl:id>
        <rdfs:label>Municipality of San Francisco del Norte</rdfs:label>
    </owl:NamedIndividual>
    


    <!-- http://purl.obolibrary.org/obo/GAZ_00066943 -->

    <owl:NamedIndividual rdf:about="http://purl.obolibrary.org/obo/GAZ_00066943">
        <rdf:type rdf:resource="http://purl.obolibrary.org/obo/ENVO_00000856"/>
        <obo:RO_0001025 rdf:resource="http://purl.obolibrary.org/obo/GAZ_00005219"/>
        <obo:IAO_0000115>A municipality in the Chinandega Department of Nicaragua.</obo:IAO_0000115>
        <oboInOwl:hasOBONamespace>GAZ</oboInOwl:hasOBONamespace>
        <oboInOwl:id>GAZ:00066943</oboInOwl:id>
        <rdfs:label>Municipality of El Viejo</rdfs:label>
    </owl:NamedIndividual>
    


    <!-- http://purl.obolibrary.org/obo/GAZ_00066944 -->

    <owl:NamedIndividual rdf:about="http://purl.obolibrary.org/obo/GAZ_00066944">
        <rdf:type rdf:resource="http://purl.obolibrary.org/obo/ENVO_00000856"/>
        <obo:RO_0001025 rdf:resource="http://purl.obolibrary.org/obo/GAZ_00005219"/>
        <obo:IAO_0000115>A municipality in the Chinandega Department of Nicaragua.</obo:IAO_0000115>
        <oboInOwl:hasOBONamespace>GAZ</oboInOwl:hasOBONamespace>
        <oboInOwl:id>GAZ:00066944</oboInOwl:id>
        <rdfs:label>Municipality of Corinto</rdfs:label>
    </owl:NamedIndividual>
    


    <!-- http://purl.obolibrary.org/obo/GAZ_00066945 -->

    <owl:NamedIndividual rdf:about="http://purl.obolibrary.org/obo/GAZ_00066945">
        <rdf:type rdf:resource="http://purl.obolibrary.org/obo/ENVO_00000856"/>
        <obo:RO_0001025 rdf:resource="http://purl.obolibrary.org/obo/GAZ_00005219"/>
        <obo:IAO_0000115>A municipality in the Chinandega Department of Nicaragua.</obo:IAO_0000115>
        <oboInOwl:hasOBONamespace>GAZ</oboInOwl:hasOBONamespace>
        <oboInOwl:id>GAZ:00066945</oboInOwl:id>
        <rdfs:label>Municipality of Somotillo</rdfs:label>
    </owl:NamedIndividual>
    


    <!-- http://purl.obolibrary.org/obo/GAZ_00066946 -->

    <owl:NamedIndividual rdf:about="http://purl.obolibrary.org/obo/GAZ_00066946">
        <rdf:type rdf:resource="http://purl.obolibrary.org/obo/ENVO_00000856"/>
        <obo:RO_0001025 rdf:resource="http://purl.obolibrary.org/obo/GAZ_00005219"/>
        <obo:IAO_0000115>A municipality in the Chinandega Department of Nicaragua.</obo:IAO_0000115>
        <oboInOwl:hasOBONamespace>GAZ</oboInOwl:hasOBONamespace>
        <oboInOwl:id>GAZ:00066946</oboInOwl:id>
        <rdfs:label>Municipality of San Pedro del Norte</rdfs:label>
    </owl:NamedIndividual>
    


    <!-- http://purl.obolibrary.org/obo/GAZ_00066947 -->

    <owl:NamedIndividual rdf:about="http://purl.obolibrary.org/obo/GAZ_00066947">
        <rdf:type rdf:resource="http://purl.obolibrary.org/obo/ENVO_00000856"/>
        <obo:RO_0001025 rdf:resource="http://purl.obolibrary.org/obo/GAZ_00005219"/>
        <obo:IAO_0000115>A municipality in the Chinandega Department of Nicaragua.</obo:IAO_0000115>
        <oboInOwl:hasOBONamespace>GAZ</oboInOwl:hasOBONamespace>
        <oboInOwl:id>GAZ:00066947</oboInOwl:id>
        <rdfs:label>Municipality of Posoltega</rdfs:label>
    </owl:NamedIndividual>
    


    <!-- http://purl.obolibrary.org/obo/GAZ_00066948 -->

    <owl:NamedIndividual rdf:about="http://purl.obolibrary.org/obo/GAZ_00066948">
        <rdf:type rdf:resource="http://purl.obolibrary.org/obo/ENVO_00000856"/>
        <obo:RO_0001025 rdf:resource="http://purl.obolibrary.org/obo/GAZ_00005219"/>
        <obo:IAO_0000115>A municipality in the Chinandega Department of Nicaragua.</obo:IAO_0000115>
        <oboInOwl:hasOBONamespace>GAZ</oboInOwl:hasOBONamespace>
        <oboInOwl:id>GAZ:00066948</oboInOwl:id>
        <rdfs:label>Municipality of Santo Tomas del Norte</rdfs:label>
    </owl:NamedIndividual>
    


    <!-- http://purl.obolibrary.org/obo/GAZ_00066949 -->

    <owl:NamedIndividual rdf:about="http://purl.obolibrary.org/obo/GAZ_00066949">
        <rdf:type rdf:resource="http://purl.obolibrary.org/obo/ENVO_00000856"/>
        <obo:RO_0001025 rdf:resource="http://purl.obolibrary.org/obo/GAZ_00005219"/>
        <obo:IAO_0000115>A municipality in the Chinandega Department of Nicaragua.</obo:IAO_0000115>
        <oboInOwl:hasOBONamespace>GAZ</oboInOwl:hasOBONamespace>
        <oboInOwl:id>GAZ:00066949</oboInOwl:id>
        <rdfs:label>Municipality of Chichigalpa</rdfs:label>
    </owl:NamedIndividual>
    


    <!-- http://purl.obolibrary.org/obo/GAZ_00066950 -->

    <owl:NamedIndividual rdf:about="http://purl.obolibrary.org/obo/GAZ_00066950">
        <rdf:type rdf:resource="http://purl.obolibrary.org/obo/ENVO_00000856"/>
        <obo:RO_0001025 rdf:resource="http://purl.obolibrary.org/obo/GAZ_00005219"/>
        <obo:IAO_0000115>A municipality in the Chinandega Department of Nicaragua.</obo:IAO_0000115>
        <oboInOwl:hasOBONamespace>GAZ</oboInOwl:hasOBONamespace>
        <oboInOwl:id>GAZ:00066950</oboInOwl:id>
        <rdfs:label>Municipality of Puerto Morazan</rdfs:label>
    </owl:NamedIndividual>
    


    <!-- http://purl.obolibrary.org/obo/GAZ_00066951 -->

    <owl:NamedIndividual rdf:about="http://purl.obolibrary.org/obo/GAZ_00066951">
        <rdf:type rdf:resource="http://purl.obolibrary.org/obo/ENVO_00000856"/>
        <obo:RO_0001025 rdf:resource="http://purl.obolibrary.org/obo/GAZ_00005219"/>
        <obo:IAO_0000115>A municipality in the Chinandega Department of Nicaragua.</obo:IAO_0000115>
        <oboInOwl:hasOBONamespace>GAZ</oboInOwl:hasOBONamespace>
        <oboInOwl:id>GAZ:00066951</oboInOwl:id>
        <rdfs:label>Municipality of El Realejo</rdfs:label>
    </owl:NamedIndividual>
    


    <!-- http://purl.obolibrary.org/obo/GAZ_00066952 -->

    <owl:NamedIndividual rdf:about="http://purl.obolibrary.org/obo/GAZ_00066952">
        <rdf:type rdf:resource="http://purl.obolibrary.org/obo/ENVO_00000856"/>
        <obo:RO_0001025 rdf:resource="http://purl.obolibrary.org/obo/GAZ_00066798"/>
        <obo:IAO_0000115>A municipality in the Chontales Department of Nicaragua.</obo:IAO_0000115>
        <oboInOwl:hasOBONamespace>GAZ</oboInOwl:hasOBONamespace>
        <oboInOwl:id>GAZ:00066952</oboInOwl:id>
        <rdfs:label>Municipality of Santo Domingo</rdfs:label>
    </owl:NamedIndividual>
    


    <!-- http://purl.obolibrary.org/obo/GAZ_00066953 -->

    <owl:NamedIndividual rdf:about="http://purl.obolibrary.org/obo/GAZ_00066953">
        <rdf:type rdf:resource="http://purl.obolibrary.org/obo/ENVO_00000856"/>
        <obo:RO_0001025 rdf:resource="http://purl.obolibrary.org/obo/GAZ_00066798"/>
        <obo:IAO_0000115>A municipality in the Chontales Department of Nicaragua.</obo:IAO_0000115>
        <oboInOwl:hasOBONamespace>GAZ</oboInOwl:hasOBONamespace>
        <oboInOwl:id>GAZ:00066953</oboInOwl:id>
        <rdfs:label>Municipality of San Pedro de Lovago</rdfs:label>
    </owl:NamedIndividual>
    


    <!-- http://purl.obolibrary.org/obo/GAZ_00066954 -->

    <owl:NamedIndividual rdf:about="http://purl.obolibrary.org/obo/GAZ_00066954">
        <rdf:type rdf:resource="http://purl.obolibrary.org/obo/ENVO_00000856"/>
        <obo:RO_0001025 rdf:resource="http://purl.obolibrary.org/obo/GAZ_00066798"/>
        <obo:IAO_0000115>A municipality in the Chontales Department of Nicaragua.</obo:IAO_0000115>
        <oboInOwl:hasOBONamespace>GAZ</oboInOwl:hasOBONamespace>
        <oboInOwl:id>GAZ:00066954</oboInOwl:id>
        <rdfs:label>Municipality of Villa Sandino</rdfs:label>
    </owl:NamedIndividual>
    


    <!-- http://purl.obolibrary.org/obo/GAZ_00066955 -->

    <owl:NamedIndividual rdf:about="http://purl.obolibrary.org/obo/GAZ_00066955">
        <rdf:type rdf:resource="http://purl.obolibrary.org/obo/ENVO_00000856"/>
        <obo:RO_0001025 rdf:resource="http://purl.obolibrary.org/obo/GAZ_00066798"/>
        <obo:IAO_0000115>A municipality in the Chontales Department of Nicaragua.</obo:IAO_0000115>
        <oboInOwl:hasOBONamespace>GAZ</oboInOwl:hasOBONamespace>
        <oboInOwl:id>GAZ:00066955</oboInOwl:id>
        <rdfs:label>Municipality of Santo Tomas</rdfs:label>
    </owl:NamedIndividual>
    


    <!-- http://purl.obolibrary.org/obo/GAZ_00066956 -->

    <owl:NamedIndividual rdf:about="http://purl.obolibrary.org/obo/GAZ_00066956">
        <rdf:type rdf:resource="http://purl.obolibrary.org/obo/ENVO_00000856"/>
        <obo:RO_0001025 rdf:resource="http://purl.obolibrary.org/obo/GAZ_00066798"/>
        <obo:IAO_0000115>A municipality in the Chontales Department of Nicaragua.</obo:IAO_0000115>
        <oboInOwl:hasOBONamespace>GAZ</oboInOwl:hasOBONamespace>
        <oboInOwl:id>GAZ:00066956</oboInOwl:id>
        <rdfs:label>Municipality of San Francisco de Cuapa</rdfs:label>
    </owl:NamedIndividual>
    


    <!-- http://purl.obolibrary.org/obo/GAZ_00066957 -->

    <owl:NamedIndividual rdf:about="http://purl.obolibrary.org/obo/GAZ_00066957">
        <rdf:type rdf:resource="http://purl.obolibrary.org/obo/ENVO_00000856"/>
        <obo:RO_0001025 rdf:resource="http://purl.obolibrary.org/obo/GAZ_00066798"/>
        <obo:IAO_0000115>A municipality in the Chontales Department of Nicaragua.</obo:IAO_0000115>
        <oboInOwl:hasOBONamespace>GAZ</oboInOwl:hasOBONamespace>
        <oboInOwl:id>GAZ:00066957</oboInOwl:id>
        <rdfs:label>Municipality of Acoyapa</rdfs:label>
    </owl:NamedIndividual>
    


    <!-- http://purl.obolibrary.org/obo/GAZ_00066958 -->

    <owl:NamedIndividual rdf:about="http://purl.obolibrary.org/obo/GAZ_00066958">
        <rdf:type rdf:resource="http://purl.obolibrary.org/obo/ENVO_00000856"/>
        <obo:RO_0001025 rdf:resource="http://purl.obolibrary.org/obo/GAZ_00066798"/>
        <obo:IAO_0000115>A municipality in the Chontales Department of Nicaragua.</obo:IAO_0000115>
        <oboInOwl:hasOBONamespace>GAZ</oboInOwl:hasOBONamespace>
        <oboInOwl:id>GAZ:00066958</oboInOwl:id>
        <rdfs:label>Municipality of El Coral</rdfs:label>
    </owl:NamedIndividual>
    


    <!-- http://purl.obolibrary.org/obo/GAZ_00066959 -->

    <owl:NamedIndividual rdf:about="http://purl.obolibrary.org/obo/GAZ_00066959">
        <rdf:type rdf:resource="http://purl.obolibrary.org/obo/ENVO_00000856"/>
        <obo:RO_0001025 rdf:resource="http://purl.obolibrary.org/obo/GAZ_00066798"/>
        <obo:IAO_0000115>A municipality in the Chontales Department of Nicaragua.</obo:IAO_0000115>
        <oboInOwl:hasOBONamespace>GAZ</oboInOwl:hasOBONamespace>
        <oboInOwl:id>GAZ:00066959</oboInOwl:id>
        <rdfs:label>Municipality of Juigalpa</rdfs:label>
    </owl:NamedIndividual>
    


    <!-- http://purl.obolibrary.org/obo/GAZ_00066960 -->

    <owl:NamedIndividual rdf:about="http://purl.obolibrary.org/obo/GAZ_00066960">
        <rdf:type rdf:resource="http://purl.obolibrary.org/obo/ENVO_00000856"/>
        <obo:RO_0001025 rdf:resource="http://purl.obolibrary.org/obo/GAZ_00066798"/>
        <obo:IAO_0000115>A municipality in the Chontales Department of Nicaragua.</obo:IAO_0000115>
        <oboInOwl:hasOBONamespace>GAZ</oboInOwl:hasOBONamespace>
        <oboInOwl:id>GAZ:00066960</oboInOwl:id>
        <rdfs:label>Municipality of La Libertad</rdfs:label>
    </owl:NamedIndividual>
    


    <!-- http://purl.obolibrary.org/obo/GAZ_00066961 -->

    <owl:NamedIndividual rdf:about="http://purl.obolibrary.org/obo/GAZ_00066961">
        <rdf:type rdf:resource="http://purl.obolibrary.org/obo/ENVO_00000856"/>
        <obo:RO_0001025 rdf:resource="http://purl.obolibrary.org/obo/GAZ_00066798"/>
        <obo:IAO_0000115>A municipality in the Chontales Department of Nicaragua.</obo:IAO_0000115>
        <oboInOwl:hasOBONamespace>GAZ</oboInOwl:hasOBONamespace>
        <oboInOwl:id>GAZ:00066961</oboInOwl:id>
        <rdfs:label>Municipality of Comalapa</rdfs:label>
    </owl:NamedIndividual>
    


    <!-- http://purl.obolibrary.org/obo/GAZ_00066962 -->

    <owl:NamedIndividual rdf:about="http://purl.obolibrary.org/obo/GAZ_00066962">
        <rdf:type rdf:resource="http://purl.obolibrary.org/obo/ENVO_00000856"/>
        <obo:RO_0001025 rdf:resource="http://purl.obolibrary.org/obo/GAZ_00056211"/>
        <obo:IAO_0000115>A municipality in the Esteli Department of Nicaragua.</obo:IAO_0000115>
        <oboInOwl:hasOBONamespace>GAZ</oboInOwl:hasOBONamespace>
        <oboInOwl:id>GAZ:00066962</oboInOwl:id>
        <rdfs:label>Municipality of Condega</rdfs:label>
    </owl:NamedIndividual>
    


    <!-- http://purl.obolibrary.org/obo/GAZ_00066963 -->

    <owl:NamedIndividual rdf:about="http://purl.obolibrary.org/obo/GAZ_00066963">
        <rdf:type rdf:resource="http://purl.obolibrary.org/obo/ENVO_00000856"/>
        <obo:RO_0001025 rdf:resource="http://purl.obolibrary.org/obo/GAZ_00056211"/>
        <obo:IAO_0000115>A municipality in the Esteli Department of Nicaragua.</obo:IAO_0000115>
        <oboInOwl:hasOBONamespace>GAZ</oboInOwl:hasOBONamespace>
        <oboInOwl:id>GAZ:00066963</oboInOwl:id>
        <rdfs:label>Municipality of San Nicolas</rdfs:label>
    </owl:NamedIndividual>
    


    <!-- http://purl.obolibrary.org/obo/GAZ_00066964 -->

    <owl:NamedIndividual rdf:about="http://purl.obolibrary.org/obo/GAZ_00066964">
        <rdf:type rdf:resource="http://purl.obolibrary.org/obo/ENVO_00000856"/>
        <obo:RO_0001025 rdf:resource="http://purl.obolibrary.org/obo/GAZ_00056211"/>
        <obo:IAO_0000115>A municipality in the Esteli Department of Nicaragua.</obo:IAO_0000115>
        <oboInOwl:hasOBONamespace>GAZ</oboInOwl:hasOBONamespace>
        <oboInOwl:id>GAZ:00066964</oboInOwl:id>
        <rdfs:label>Municipality of Esteli</rdfs:label>
    </owl:NamedIndividual>
    


    <!-- http://purl.obolibrary.org/obo/GAZ_00066965 -->

    <owl:NamedIndividual rdf:about="http://purl.obolibrary.org/obo/GAZ_00066965">
        <rdf:type rdf:resource="http://purl.obolibrary.org/obo/ENVO_00000856"/>
        <obo:RO_0001025 rdf:resource="http://purl.obolibrary.org/obo/GAZ_00056211"/>
        <obo:IAO_0000115>A municipality in the Esteli Department of Nicaragua.</obo:IAO_0000115>
        <oboInOwl:hasOBONamespace>GAZ</oboInOwl:hasOBONamespace>
        <oboInOwl:id>GAZ:00066965</oboInOwl:id>
        <rdfs:label>Municipality of Pueblo Nuevo</rdfs:label>
    </owl:NamedIndividual>
    


    <!-- http://purl.obolibrary.org/obo/GAZ_00066966 -->

    <owl:NamedIndividual rdf:about="http://purl.obolibrary.org/obo/GAZ_00066966">
        <rdf:type rdf:resource="http://purl.obolibrary.org/obo/ENVO_00000856"/>
        <obo:RO_0001025 rdf:resource="http://purl.obolibrary.org/obo/GAZ_00056211"/>
        <obo:IAO_0000115>A municipality in the Esteli Department of Nicaragua.</obo:IAO_0000115>
        <oboInOwl:hasOBONamespace>GAZ</oboInOwl:hasOBONamespace>
        <oboInOwl:id>GAZ:00066966</oboInOwl:id>
        <rdfs:label>Municipality of San Juan de Limay</rdfs:label>
    </owl:NamedIndividual>
    


    <!-- http://purl.obolibrary.org/obo/GAZ_00066967 -->

    <owl:NamedIndividual rdf:about="http://purl.obolibrary.org/obo/GAZ_00066967">
        <rdf:type rdf:resource="http://purl.obolibrary.org/obo/ENVO_00000856"/>
        <obo:RO_0001025 rdf:resource="http://purl.obolibrary.org/obo/GAZ_00056211"/>
        <obo:IAO_0000115>A municipality in the Esteli Department of Nicaragua.</obo:IAO_0000115>
        <oboInOwl:hasOBONamespace>GAZ</oboInOwl:hasOBONamespace>
        <oboInOwl:id>GAZ:00066967</oboInOwl:id>
        <rdfs:label>Municipality of La Trinidad</rdfs:label>
    </owl:NamedIndividual>
    


    <!-- http://purl.obolibrary.org/obo/GAZ_00066968 -->

    <owl:NamedIndividual rdf:about="http://purl.obolibrary.org/obo/GAZ_00066968">
        <rdf:type rdf:resource="http://purl.obolibrary.org/obo/ENVO_00000856"/>
        <obo:RO_0001025 rdf:resource="http://purl.obolibrary.org/obo/GAZ_00056204"/>
        <obo:IAO_0000115>A municipality in the Granada Department of Nicaragua.</obo:IAO_0000115>
        <oboInOwl:hasOBONamespace>GAZ</oboInOwl:hasOBONamespace>
        <oboInOwl:id>GAZ:00066968</oboInOwl:id>
        <rdfs:label>Municipality of Diria</rdfs:label>
    </owl:NamedIndividual>
    


    <!-- http://purl.obolibrary.org/obo/GAZ_00066969 -->

    <owl:NamedIndividual rdf:about="http://purl.obolibrary.org/obo/GAZ_00066969">
        <rdf:type rdf:resource="http://purl.obolibrary.org/obo/ENVO_00000856"/>
        <obo:RO_0001025 rdf:resource="http://purl.obolibrary.org/obo/GAZ_00056204"/>
        <obo:IAO_0000115>A municipality in the Granada Department of Nicaragua.</obo:IAO_0000115>
        <oboInOwl:hasOBONamespace>GAZ</oboInOwl:hasOBONamespace>
        <oboInOwl:id>GAZ:00066969</oboInOwl:id>
        <rdfs:label>Municipality of Nandaime</rdfs:label>
    </owl:NamedIndividual>
    


    <!-- http://purl.obolibrary.org/obo/GAZ_00066970 -->

    <owl:NamedIndividual rdf:about="http://purl.obolibrary.org/obo/GAZ_00066970">
        <rdf:type rdf:resource="http://purl.obolibrary.org/obo/ENVO_00000856"/>
        <obo:RO_0001025 rdf:resource="http://purl.obolibrary.org/obo/GAZ_00056204"/>
        <obo:IAO_0000115>A municipality in the Granada Department of Nicaragua.</obo:IAO_0000115>
        <oboInOwl:hasOBONamespace>GAZ</oboInOwl:hasOBONamespace>
        <oboInOwl:id>GAZ:00066970</oboInOwl:id>
        <rdfs:label>Municipality of Granada</rdfs:label>
    </owl:NamedIndividual>
    


    <!-- http://purl.obolibrary.org/obo/GAZ_00066971 -->

    <owl:NamedIndividual rdf:about="http://purl.obolibrary.org/obo/GAZ_00066971">
        <rdf:type rdf:resource="http://purl.obolibrary.org/obo/ENVO_00000856"/>
        <obo:RO_0001025 rdf:resource="http://purl.obolibrary.org/obo/GAZ_00056204"/>
        <obo:IAO_0000115>A municipality in the Granada Department of Nicaragua.</obo:IAO_0000115>
        <oboInOwl:hasOBONamespace>GAZ</oboInOwl:hasOBONamespace>
        <oboInOwl:id>GAZ:00066971</oboInOwl:id>
        <rdfs:label>Municipality of Diriomo</rdfs:label>
    </owl:NamedIndividual>
    


    <!-- http://purl.obolibrary.org/obo/GAZ_00066972 -->

    <owl:NamedIndividual rdf:about="http://purl.obolibrary.org/obo/GAZ_00066972">
        <rdf:type rdf:resource="http://purl.obolibrary.org/obo/ENVO_00000856"/>
        <obo:RO_0001025 rdf:resource="http://purl.obolibrary.org/obo/GAZ_00062427"/>
        <obo:IAO_0000115>A municipality in the Jinotega Department of Nicaragua.</obo:IAO_0000115>
        <oboInOwl:hasOBONamespace>GAZ</oboInOwl:hasOBONamespace>
        <oboInOwl:id>GAZ:00066972</oboInOwl:id>
        <rdfs:label>Municipality of San Sebastian de Yali</rdfs:label>
    </owl:NamedIndividual>
    


    <!-- http://purl.obolibrary.org/obo/GAZ_00066973 -->

    <owl:NamedIndividual rdf:about="http://purl.obolibrary.org/obo/GAZ_00066973">
        <rdf:type rdf:resource="http://purl.obolibrary.org/obo/ENVO_00000856"/>
        <obo:RO_0001025 rdf:resource="http://purl.obolibrary.org/obo/GAZ_00062427"/>
        <obo:IAO_0000115>A municipality in the Jinotega Department of Nicaragua.</obo:IAO_0000115>
        <oboInOwl:hasOBONamespace>GAZ</oboInOwl:hasOBONamespace>
        <oboInOwl:id>GAZ:00066973</oboInOwl:id>
        <rdfs:label>Municipality of Wiwili</rdfs:label>
    </owl:NamedIndividual>
    


    <!-- http://purl.obolibrary.org/obo/GAZ_00066974 -->

    <owl:NamedIndividual rdf:about="http://purl.obolibrary.org/obo/GAZ_00066974">
        <rdf:type rdf:resource="http://purl.obolibrary.org/obo/ENVO_00000856"/>
        <obo:RO_0001025 rdf:resource="http://purl.obolibrary.org/obo/GAZ_00062427"/>
        <obo:IAO_0000115>A municipality in the Jinotega Department of Nicaragua.</obo:IAO_0000115>
        <oboInOwl:hasOBONamespace>GAZ</oboInOwl:hasOBONamespace>
        <oboInOwl:id>GAZ:00066974</oboInOwl:id>
        <rdfs:label>Municipality of San Jose de Bocay</rdfs:label>
    </owl:NamedIndividual>
    


    <!-- http://purl.obolibrary.org/obo/GAZ_00066975 -->

    <owl:NamedIndividual rdf:about="http://purl.obolibrary.org/obo/GAZ_00066975">
        <rdf:type rdf:resource="http://purl.obolibrary.org/obo/ENVO_00000856"/>
        <obo:RO_0001025 rdf:resource="http://purl.obolibrary.org/obo/GAZ_00062427"/>
        <obo:IAO_0000115>A municipality in the Jinotega Department of Nicaragua.</obo:IAO_0000115>
        <oboInOwl:hasOBONamespace>GAZ</oboInOwl:hasOBONamespace>
        <oboInOwl:id>GAZ:00066975</oboInOwl:id>
        <rdfs:label>Municipality of Jinotega</rdfs:label>
    </owl:NamedIndividual>
    


    <!-- http://purl.obolibrary.org/obo/GAZ_00066976 -->

    <owl:NamedIndividual rdf:about="http://purl.obolibrary.org/obo/GAZ_00066976">
        <rdf:type rdf:resource="http://purl.obolibrary.org/obo/ENVO_00000856"/>
        <obo:RO_0001025 rdf:resource="http://purl.obolibrary.org/obo/GAZ_00062427"/>
        <obo:IAO_0000115>A municipality in the Jinotega Department of Nicaragua.</obo:IAO_0000115>
        <oboInOwl:hasOBONamespace>GAZ</oboInOwl:hasOBONamespace>
        <oboInOwl:id>GAZ:00066976</oboInOwl:id>
        <rdfs:label>Municipality of Santa Maria de Pantasma</rdfs:label>
    </owl:NamedIndividual>
    


    <!-- http://purl.obolibrary.org/obo/GAZ_00066977 -->

    <owl:NamedIndividual rdf:about="http://purl.obolibrary.org/obo/GAZ_00066977">
        <rdf:type rdf:resource="http://purl.obolibrary.org/obo/ENVO_00000856"/>
        <obo:RO_0001025 rdf:resource="http://purl.obolibrary.org/obo/GAZ_00062427"/>
        <obo:IAO_0000115>A municipality in the Jinotega Department of Nicaragua.</obo:IAO_0000115>
        <oboInOwl:hasOBONamespace>GAZ</oboInOwl:hasOBONamespace>
        <oboInOwl:id>GAZ:00066977</oboInOwl:id>
        <rdfs:label>Municipality of La Concordia</rdfs:label>
    </owl:NamedIndividual>
    


    <!-- http://purl.obolibrary.org/obo/GAZ_00066978 -->

    <owl:NamedIndividual rdf:about="http://purl.obolibrary.org/obo/GAZ_00066978">
        <rdf:type rdf:resource="http://purl.obolibrary.org/obo/ENVO_00000856"/>
        <obo:RO_0001025 rdf:resource="http://purl.obolibrary.org/obo/GAZ_00062427"/>
        <obo:IAO_0000115>A municipality in the Jinotega Department of Nicaragua.</obo:IAO_0000115>
        <oboInOwl:hasOBONamespace>GAZ</oboInOwl:hasOBONamespace>
        <oboInOwl:id>GAZ:00066978</oboInOwl:id>
        <rdfs:label>Municipality of San Rafael del Norte</rdfs:label>
    </owl:NamedIndividual>
    


    <!-- http://purl.obolibrary.org/obo/GAZ_00066979 -->

    <owl:NamedIndividual rdf:about="http://purl.obolibrary.org/obo/GAZ_00066979">
        <rdf:type rdf:resource="http://purl.obolibrary.org/obo/ENVO_00000856"/>
        <obo:RO_0001025 rdf:resource="http://purl.obolibrary.org/obo/GAZ_00062427"/>
        <obo:IAO_0000115>A municipality in the Jinotega Department of Nicaragua.</obo:IAO_0000115>
        <oboInOwl:hasOBONamespace>GAZ</oboInOwl:hasOBONamespace>
        <oboInOwl:id>GAZ:00066979</oboInOwl:id>
        <rdfs:label>Municipality of El Cua</rdfs:label>
    </owl:NamedIndividual>
    


    <!-- http://purl.obolibrary.org/obo/GAZ_00066980 -->

    <owl:NamedIndividual rdf:about="http://purl.obolibrary.org/obo/GAZ_00066980">
        <rdf:type rdf:resource="http://purl.obolibrary.org/obo/ENVO_00000856"/>
        <obo:RO_0001025 rdf:resource="http://purl.obolibrary.org/obo/GAZ_00056193"/>
        <obo:IAO_0000115>A municipality in the Leon Department of Nicaragua.</obo:IAO_0000115>
        <oboInOwl:hasOBONamespace>GAZ</oboInOwl:hasOBONamespace>
        <oboInOwl:id>GAZ:00066980</oboInOwl:id>
        <rdfs:label>Municipality of La Paz Centro</rdfs:label>
    </owl:NamedIndividual>
    


    <!-- http://purl.obolibrary.org/obo/GAZ_00066981 -->

    <owl:NamedIndividual rdf:about="http://purl.obolibrary.org/obo/GAZ_00066981">
        <rdf:type rdf:resource="http://purl.obolibrary.org/obo/ENVO_00000856"/>
        <obo:RO_0001025 rdf:resource="http://purl.obolibrary.org/obo/GAZ_00056193"/>
        <obo:IAO_0000115>A municipality in the Leon Department of Nicaragua.</obo:IAO_0000115>
        <oboInOwl:hasOBONamespace>GAZ</oboInOwl:hasOBONamespace>
        <oboInOwl:id>GAZ:00066981</oboInOwl:id>
        <rdfs:label>Municipality of San Jose de Achuapa</rdfs:label>
    </owl:NamedIndividual>
    


    <!-- http://purl.obolibrary.org/obo/GAZ_00066982 -->

    <owl:NamedIndividual rdf:about="http://purl.obolibrary.org/obo/GAZ_00066982">
        <rdf:type rdf:resource="http://purl.obolibrary.org/obo/ENVO_00000856"/>
        <obo:RO_0001025 rdf:resource="http://purl.obolibrary.org/obo/GAZ_00056193"/>
        <obo:IAO_0000115>A municipality in the Leon Department of Nicaragua.</obo:IAO_0000115>
        <oboInOwl:hasOBONamespace>GAZ</oboInOwl:hasOBONamespace>
        <oboInOwl:id>GAZ:00066982</oboInOwl:id>
        <rdfs:label>Municipality of Telica</rdfs:label>
    </owl:NamedIndividual>
    


    <!-- http://purl.obolibrary.org/obo/GAZ_00066983 -->

    <owl:NamedIndividual rdf:about="http://purl.obolibrary.org/obo/GAZ_00066983">
        <rdf:type rdf:resource="http://purl.obolibrary.org/obo/ENVO_00000856"/>
        <obo:RO_0001025 rdf:resource="http://purl.obolibrary.org/obo/GAZ_00056193"/>
        <obo:IAO_0000115>A municipality in the Leon Department of Nicaragua.</obo:IAO_0000115>
        <oboInOwl:hasOBONamespace>GAZ</oboInOwl:hasOBONamespace>
        <oboInOwl:id>GAZ:00066983</oboInOwl:id>
        <rdfs:label>Municipality of Santa Rosa del Penon</rdfs:label>
    </owl:NamedIndividual>
    


    <!-- http://purl.obolibrary.org/obo/GAZ_00066984 -->

    <owl:NamedIndividual rdf:about="http://purl.obolibrary.org/obo/GAZ_00066984">
        <rdf:type rdf:resource="http://purl.obolibrary.org/obo/ENVO_00000856"/>
        <obo:RO_0001025 rdf:resource="http://purl.obolibrary.org/obo/GAZ_00056193"/>
        <obo:IAO_0000115>A municipality in the Leon Department of Nicaragua.</obo:IAO_0000115>
        <oboInOwl:hasOBONamespace>GAZ</oboInOwl:hasOBONamespace>
        <oboInOwl:id>GAZ:00066984</oboInOwl:id>
        <rdfs:label>Municipality of El Jicaral</rdfs:label>
    </owl:NamedIndividual>
    


    <!-- http://purl.obolibrary.org/obo/GAZ_00066985 -->

    <owl:NamedIndividual rdf:about="http://purl.obolibrary.org/obo/GAZ_00066985">
        <rdf:type rdf:resource="http://purl.obolibrary.org/obo/ENVO_00000856"/>
        <obo:RO_0001025 rdf:resource="http://purl.obolibrary.org/obo/GAZ_00056193"/>
        <obo:IAO_0000115>A municipality in the Leon Department of Nicaragua.</obo:IAO_0000115>
        <oboInOwl:hasOBONamespace>GAZ</oboInOwl:hasOBONamespace>
        <oboInOwl:id>GAZ:00066985</oboInOwl:id>
        <rdfs:label>Municipality of Larreynaga</rdfs:label>
    </owl:NamedIndividual>
    


    <!-- http://purl.obolibrary.org/obo/GAZ_00066986 -->

    <owl:NamedIndividual rdf:about="http://purl.obolibrary.org/obo/GAZ_00066986">
        <rdf:type rdf:resource="http://purl.obolibrary.org/obo/ENVO_00000856"/>
        <obo:RO_0001025 rdf:resource="http://purl.obolibrary.org/obo/GAZ_00056193"/>
        <obo:IAO_0000115>A municipality in the Leon Department of Nicaragua.</obo:IAO_0000115>
        <oboInOwl:hasOBONamespace>GAZ</oboInOwl:hasOBONamespace>
        <oboInOwl:id>GAZ:00066986</oboInOwl:id>
        <rdfs:label>Municipality of Nagarote</rdfs:label>
    </owl:NamedIndividual>
    


    <!-- http://purl.obolibrary.org/obo/GAZ_00066987 -->

    <owl:NamedIndividual rdf:about="http://purl.obolibrary.org/obo/GAZ_00066987">
        <rdf:type rdf:resource="http://purl.obolibrary.org/obo/ENVO_00000856"/>
        <obo:RO_0001025 rdf:resource="http://purl.obolibrary.org/obo/GAZ_00056193"/>
        <obo:IAO_0000115>A municipality in the Leon Department of Nicaragua.</obo:IAO_0000115>
        <oboInOwl:hasOBONamespace>GAZ</oboInOwl:hasOBONamespace>
        <oboInOwl:id>GAZ:00066987</oboInOwl:id>
        <rdfs:label>Municipality of Leon</rdfs:label>
    </owl:NamedIndividual>
    


    <!-- http://purl.obolibrary.org/obo/GAZ_00066988 -->

    <owl:NamedIndividual rdf:about="http://purl.obolibrary.org/obo/GAZ_00066988">
        <rdf:type rdf:resource="http://purl.obolibrary.org/obo/ENVO_00000856"/>
        <obo:RO_0001025 rdf:resource="http://purl.obolibrary.org/obo/GAZ_00056193"/>
        <obo:IAO_0000115>A municipality in the Leon Department of Nicaragua.</obo:IAO_0000115>
        <oboInOwl:hasOBONamespace>GAZ</oboInOwl:hasOBONamespace>
        <oboInOwl:id>GAZ:00066988</oboInOwl:id>
        <rdfs:label>Municipality of El Sauce</rdfs:label>
    </owl:NamedIndividual>
    


    <!-- http://purl.obolibrary.org/obo/GAZ_00066989 -->

    <owl:NamedIndividual rdf:about="http://purl.obolibrary.org/obo/GAZ_00066989">
        <rdf:type rdf:resource="http://purl.obolibrary.org/obo/ENVO_00000856"/>
        <obo:RO_0001025 rdf:resource="http://purl.obolibrary.org/obo/GAZ_00056193"/>
        <obo:IAO_0000115>A municipality in the Leon Department of Nicaragua.</obo:IAO_0000115>
        <oboInOwl:hasOBONamespace>GAZ</oboInOwl:hasOBONamespace>
        <oboInOwl:id>GAZ:00066989</oboInOwl:id>
        <rdfs:label>Municipality of Quezalguaque</rdfs:label>
    </owl:NamedIndividual>
    


    <!-- http://purl.obolibrary.org/obo/GAZ_00066990 -->

    <owl:NamedIndividual rdf:about="http://purl.obolibrary.org/obo/GAZ_00066990">
        <rdf:type rdf:resource="http://purl.obolibrary.org/obo/ENVO_00000856"/>
        <obo:RO_0001025 rdf:resource="http://purl.obolibrary.org/obo/GAZ_00066803"/>
        <obo:IAO_0000115>A municipality in the Madriz Department of Nicaragua.</obo:IAO_0000115>
        <oboInOwl:hasOBONamespace>GAZ</oboInOwl:hasOBONamespace>
        <oboInOwl:id>GAZ:00066990</oboInOwl:id>
        <rdfs:label>Municipality of Somoto</rdfs:label>
    </owl:NamedIndividual>
    


    <!-- http://purl.obolibrary.org/obo/GAZ_00066991 -->

    <owl:NamedIndividual rdf:about="http://purl.obolibrary.org/obo/GAZ_00066991">
        <rdf:type rdf:resource="http://purl.obolibrary.org/obo/ENVO_00000856"/>
        <obo:RO_0001025 rdf:resource="http://purl.obolibrary.org/obo/GAZ_00066803"/>
        <obo:IAO_0000115>A municipality in the Madriz Department of Nicaragua.</obo:IAO_0000115>
        <oboInOwl:hasOBONamespace>GAZ</oboInOwl:hasOBONamespace>
        <oboInOwl:id>GAZ:00066991</oboInOwl:id>
        <rdfs:label>Municipality of Totogalpa</rdfs:label>
    </owl:NamedIndividual>
    


    <!-- http://purl.obolibrary.org/obo/GAZ_00066992 -->

    <owl:NamedIndividual rdf:about="http://purl.obolibrary.org/obo/GAZ_00066992">
        <rdf:type rdf:resource="http://purl.obolibrary.org/obo/ENVO_00000856"/>
        <obo:RO_0001025 rdf:resource="http://purl.obolibrary.org/obo/GAZ_00066803"/>
        <obo:IAO_0000115>A municipality in the Madriz Department of Nicaragua.</obo:IAO_0000115>
        <oboInOwl:hasOBONamespace>GAZ</oboInOwl:hasOBONamespace>
        <oboInOwl:id>GAZ:00066992</oboInOwl:id>
        <rdfs:label>Municipality of Yalaguina</rdfs:label>
    </owl:NamedIndividual>
    


    <!-- http://purl.obolibrary.org/obo/GAZ_00066993 -->

    <owl:NamedIndividual rdf:about="http://purl.obolibrary.org/obo/GAZ_00066993">
        <rdf:type rdf:resource="http://purl.obolibrary.org/obo/ENVO_00000856"/>
        <obo:RO_0001025 rdf:resource="http://purl.obolibrary.org/obo/GAZ_00066803"/>
        <obo:IAO_0000115>A municipality in the Madriz Department of Nicaragua.</obo:IAO_0000115>
        <oboInOwl:hasOBONamespace>GAZ</oboInOwl:hasOBONamespace>
        <oboInOwl:id>GAZ:00066993</oboInOwl:id>
        <rdfs:label>Municipality of Telpaneca</rdfs:label>
    </owl:NamedIndividual>
    


    <!-- http://purl.obolibrary.org/obo/GAZ_00066994 -->

    <owl:NamedIndividual rdf:about="http://purl.obolibrary.org/obo/GAZ_00066994">
        <rdf:type rdf:resource="http://purl.obolibrary.org/obo/ENVO_00000856"/>
        <obo:RO_0001025 rdf:resource="http://purl.obolibrary.org/obo/GAZ_00066803"/>
        <obo:IAO_0000115>A municipality in the Madriz Department of Nicaragua.</obo:IAO_0000115>
        <oboInOwl:hasOBONamespace>GAZ</oboInOwl:hasOBONamespace>
        <oboInOwl:id>GAZ:00066994</oboInOwl:id>
        <rdfs:label>Municipality of San Juan del Rio Coco</rdfs:label>
    </owl:NamedIndividual>
    


    <!-- http://purl.obolibrary.org/obo/GAZ_00066995 -->

    <owl:NamedIndividual rdf:about="http://purl.obolibrary.org/obo/GAZ_00066995">
        <rdf:type rdf:resource="http://purl.obolibrary.org/obo/ENVO_00000856"/>
        <obo:RO_0001025 rdf:resource="http://purl.obolibrary.org/obo/GAZ_00066803"/>
        <obo:IAO_0000115>A municipality in the Madriz Department of Nicaragua.</obo:IAO_0000115>
        <oboInOwl:hasOBONamespace>GAZ</oboInOwl:hasOBONamespace>
        <oboInOwl:id>GAZ:00066995</oboInOwl:id>
        <rdfs:label>Municipality of San Jose de Cusmapa</rdfs:label>
    </owl:NamedIndividual>
    


    <!-- http://purl.obolibrary.org/obo/GAZ_00066996 -->

    <owl:NamedIndividual rdf:about="http://purl.obolibrary.org/obo/GAZ_00066996">
        <rdf:type rdf:resource="http://purl.obolibrary.org/obo/ENVO_00000856"/>
        <obo:RO_0001025 rdf:resource="http://purl.obolibrary.org/obo/GAZ_00066803"/>
        <obo:IAO_0000115>A municipality in the Madriz Department of Nicaragua.</obo:IAO_0000115>
        <oboInOwl:hasOBONamespace>GAZ</oboInOwl:hasOBONamespace>
        <oboInOwl:id>GAZ:00066996</oboInOwl:id>
        <rdfs:label>Municipality of Las Sabanas</rdfs:label>
    </owl:NamedIndividual>
    


    <!-- http://purl.obolibrary.org/obo/GAZ_00066997 -->

    <owl:NamedIndividual rdf:about="http://purl.obolibrary.org/obo/GAZ_00066997">
        <rdf:type rdf:resource="http://purl.obolibrary.org/obo/ENVO_00000856"/>
        <obo:RO_0001025 rdf:resource="http://purl.obolibrary.org/obo/GAZ_00066803"/>
        <obo:IAO_0000115>A municipality in the Madriz Department of Nicaragua.</obo:IAO_0000115>
        <oboInOwl:hasOBONamespace>GAZ</oboInOwl:hasOBONamespace>
        <oboInOwl:id>GAZ:00066997</oboInOwl:id>
        <rdfs:label>Municipality of Palacaguina</rdfs:label>
    </owl:NamedIndividual>
    


    <!-- http://purl.obolibrary.org/obo/GAZ_00066998 -->

    <owl:NamedIndividual rdf:about="http://purl.obolibrary.org/obo/GAZ_00066998">
        <rdf:type rdf:resource="http://purl.obolibrary.org/obo/ENVO_00000856"/>
        <obo:RO_0001025 rdf:resource="http://purl.obolibrary.org/obo/GAZ_00066803"/>
        <obo:IAO_0000115>A municipality in the Madriz Department of Nicaragua.</obo:IAO_0000115>
        <oboInOwl:hasOBONamespace>GAZ</oboInOwl:hasOBONamespace>
        <oboInOwl:id>GAZ:00066998</oboInOwl:id>
        <rdfs:label>Municipality of San Lucas</rdfs:label>
    </owl:NamedIndividual>
    


    <!-- http://purl.obolibrary.org/obo/GAZ_00066999 -->

    <owl:NamedIndividual rdf:about="http://purl.obolibrary.org/obo/GAZ_00066999">
        <rdf:type rdf:resource="http://purl.obolibrary.org/obo/ENVO_00000856"/>
        <obo:RO_0001025 rdf:resource="http://purl.obolibrary.org/obo/GAZ_00066801"/>
        <obo:IAO_0000115>A municipality in the Managua Department of Nicaragua.</obo:IAO_0000115>
        <oboInOwl:hasOBONamespace>GAZ</oboInOwl:hasOBONamespace>
        <oboInOwl:id>GAZ:00066999</oboInOwl:id>
        <rdfs:label>Municipality of San Rafael del Sur</rdfs:label>
    </owl:NamedIndividual>
    


    <!-- http://purl.obolibrary.org/obo/GAZ_00067000 -->

    <owl:NamedIndividual rdf:about="http://purl.obolibrary.org/obo/GAZ_00067000">
        <rdf:type rdf:resource="http://purl.obolibrary.org/obo/ENVO_00000856"/>
        <obo:RO_0001025 rdf:resource="http://purl.obolibrary.org/obo/GAZ_00066801"/>
        <obo:IAO_0000115>A municipality in the Managua Department of Nicaragua.</obo:IAO_0000115>
        <oboInOwl:hasOBONamespace>GAZ</oboInOwl:hasOBONamespace>
        <oboInOwl:id>GAZ:00067000</oboInOwl:id>
        <rdfs:label>Municipality of El Crucero</rdfs:label>
    </owl:NamedIndividual>
    


    <!-- http://purl.obolibrary.org/obo/GAZ_00067001 -->

    <owl:NamedIndividual rdf:about="http://purl.obolibrary.org/obo/GAZ_00067001">
        <rdf:type rdf:resource="http://purl.obolibrary.org/obo/ENVO_00000856"/>
        <obo:RO_0001025 rdf:resource="http://purl.obolibrary.org/obo/GAZ_00066801"/>
        <obo:IAO_0000115>A municipality in the Managua Department of Nicaragua.</obo:IAO_0000115>
        <oboInOwl:hasOBONamespace>GAZ</oboInOwl:hasOBONamespace>
        <oboInOwl:id>GAZ:00067001</oboInOwl:id>
        <rdfs:label>Municipality of Villa Carlos Fonseca</rdfs:label>
    </owl:NamedIndividual>
    


    <!-- http://purl.obolibrary.org/obo/GAZ_00067002 -->

    <owl:NamedIndividual rdf:about="http://purl.obolibrary.org/obo/GAZ_00067002">
        <rdf:type rdf:resource="http://purl.obolibrary.org/obo/ENVO_00000856"/>
        <obo:RO_0001025 rdf:resource="http://purl.obolibrary.org/obo/GAZ_00066801"/>
        <obo:IAO_0000115>A municipality in the Managua Department of Nicaragua.</obo:IAO_0000115>
        <oboInOwl:hasOBONamespace>GAZ</oboInOwl:hasOBONamespace>
        <oboInOwl:id>GAZ:00067002</oboInOwl:id>
        <rdfs:label>Municipality of Tipitapa</rdfs:label>
    </owl:NamedIndividual>
    


    <!-- http://purl.obolibrary.org/obo/GAZ_00067003 -->

    <owl:NamedIndividual rdf:about="http://purl.obolibrary.org/obo/GAZ_00067003">
        <rdf:type rdf:resource="http://purl.obolibrary.org/obo/ENVO_00000856"/>
        <obo:RO_0001025 rdf:resource="http://purl.obolibrary.org/obo/GAZ_00066801"/>
        <obo:IAO_0000115>A municipality in the Managua Department of Nicaragua.</obo:IAO_0000115>
        <oboInOwl:hasOBONamespace>GAZ</oboInOwl:hasOBONamespace>
        <oboInOwl:id>GAZ:00067003</oboInOwl:id>
        <rdfs:label>Municipality of San Francisco Libre</rdfs:label>
    </owl:NamedIndividual>
    


    <!-- http://purl.obolibrary.org/obo/GAZ_00067004 -->

    <owl:NamedIndividual rdf:about="http://purl.obolibrary.org/obo/GAZ_00067004">
        <rdf:type rdf:resource="http://purl.obolibrary.org/obo/ENVO_00000856"/>
        <obo:RO_0001025 rdf:resource="http://purl.obolibrary.org/obo/GAZ_00066801"/>
        <obo:IAO_0000115>A municipality in the Managua Department of Nicaragua.</obo:IAO_0000115>
        <oboInOwl:hasOBONamespace>GAZ</oboInOwl:hasOBONamespace>
        <oboInOwl:id>GAZ:00067004</oboInOwl:id>
        <rdfs:label>Municipality of Managua</rdfs:label>
    </owl:NamedIndividual>
    


    <!-- http://purl.obolibrary.org/obo/GAZ_00067005 -->

    <owl:NamedIndividual rdf:about="http://purl.obolibrary.org/obo/GAZ_00067005">
        <rdf:type rdf:resource="http://purl.obolibrary.org/obo/ENVO_00000856"/>
        <obo:RO_0001025 rdf:resource="http://purl.obolibrary.org/obo/GAZ_00066801"/>
        <obo:IAO_0000115>A municipality in the Managua Department of Nicaragua.</obo:IAO_0000115>
        <oboInOwl:hasOBONamespace>GAZ</oboInOwl:hasOBONamespace>
        <oboInOwl:id>GAZ:00067005</oboInOwl:id>
        <rdfs:label>Municipality of Ciudad Sandino</rdfs:label>
    </owl:NamedIndividual>
    


    <!-- http://purl.obolibrary.org/obo/GAZ_00067006 -->

    <owl:NamedIndividual rdf:about="http://purl.obolibrary.org/obo/GAZ_00067006">
        <rdf:type rdf:resource="http://purl.obolibrary.org/obo/ENVO_00000856"/>
        <obo:RO_0001025 rdf:resource="http://purl.obolibrary.org/obo/GAZ_00066801"/>
        <obo:IAO_0000115>A municipality in the Managua Department of Nicaragua.</obo:IAO_0000115>
        <oboInOwl:hasOBONamespace>GAZ</oboInOwl:hasOBONamespace>
        <oboInOwl:id>GAZ:00067006</oboInOwl:id>
        <rdfs:label>Municipality of Ticuantepe</rdfs:label>
    </owl:NamedIndividual>
    


    <!-- http://purl.obolibrary.org/obo/GAZ_00067007 -->

    <owl:NamedIndividual rdf:about="http://purl.obolibrary.org/obo/GAZ_00067007">
        <rdf:type rdf:resource="http://purl.obolibrary.org/obo/ENVO_00000856"/>
        <obo:RO_0001025 rdf:resource="http://purl.obolibrary.org/obo/GAZ_00066801"/>
        <obo:IAO_0000115>A municipality in the Managua Department of Nicaragua.</obo:IAO_0000115>
        <oboInOwl:hasOBONamespace>GAZ</oboInOwl:hasOBONamespace>
        <oboInOwl:id>GAZ:00067007</oboInOwl:id>
        <rdfs:label>Municipality of Mateare</rdfs:label>
    </owl:NamedIndividual>
    


    <!-- http://purl.obolibrary.org/obo/GAZ_00067008 -->

    <owl:NamedIndividual rdf:about="http://purl.obolibrary.org/obo/GAZ_00067008">
        <rdf:type rdf:resource="http://purl.obolibrary.org/obo/ENVO_00000856"/>
        <obo:RO_0001025 rdf:resource="http://purl.obolibrary.org/obo/GAZ_00056201"/>
        <obo:IAO_0000115>A municipality in the Masaya Department of Nicaragua.</obo:IAO_0000115>
        <oboInOwl:hasOBONamespace>GAZ</oboInOwl:hasOBONamespace>
        <oboInOwl:id>GAZ:00067008</oboInOwl:id>
        <rdfs:label>Municipality of Nindiri</rdfs:label>
    </owl:NamedIndividual>
    


    <!-- http://purl.obolibrary.org/obo/GAZ_00067009 -->

    <owl:NamedIndividual rdf:about="http://purl.obolibrary.org/obo/GAZ_00067009">
        <rdf:type rdf:resource="http://purl.obolibrary.org/obo/ENVO_00000856"/>
        <obo:RO_0001025 rdf:resource="http://purl.obolibrary.org/obo/GAZ_00056201"/>
        <obo:IAO_0000115>A municipality in the Masaya Department of Nicaragua.</obo:IAO_0000115>
        <oboInOwl:hasOBONamespace>GAZ</oboInOwl:hasOBONamespace>
        <oboInOwl:id>GAZ:00067009</oboInOwl:id>
        <rdfs:label>Municipality of Tisma</rdfs:label>
    </owl:NamedIndividual>
    


    <!-- http://purl.obolibrary.org/obo/GAZ_00067010 -->

    <owl:NamedIndividual rdf:about="http://purl.obolibrary.org/obo/GAZ_00067010">
        <rdf:type rdf:resource="http://purl.obolibrary.org/obo/ENVO_00000856"/>
        <obo:RO_0001025 rdf:resource="http://purl.obolibrary.org/obo/GAZ_00056201"/>
        <obo:IAO_0000115>A municipality in the Masaya Department of Nicaragua.</obo:IAO_0000115>
        <oboInOwl:hasOBONamespace>GAZ</oboInOwl:hasOBONamespace>
        <oboInOwl:id>GAZ:00067010</oboInOwl:id>
        <rdfs:label>Municipality of San Juan de Oriente</rdfs:label>
    </owl:NamedIndividual>
    


    <!-- http://purl.obolibrary.org/obo/GAZ_00067011 -->

    <owl:NamedIndividual rdf:about="http://purl.obolibrary.org/obo/GAZ_00067011">
        <rdf:type rdf:resource="http://purl.obolibrary.org/obo/ENVO_00000856"/>
        <obo:RO_0001025 rdf:resource="http://purl.obolibrary.org/obo/GAZ_00056201"/>
        <obo:IAO_0000115>A municipality in the Masaya Department of Nicaragua.</obo:IAO_0000115>
        <oboInOwl:hasOBONamespace>GAZ</oboInOwl:hasOBONamespace>
        <oboInOwl:id>GAZ:00067011</oboInOwl:id>
        <rdfs:label>Municipality of Masatepe</rdfs:label>
    </owl:NamedIndividual>
    


    <!-- http://purl.obolibrary.org/obo/GAZ_00067012 -->

    <owl:NamedIndividual rdf:about="http://purl.obolibrary.org/obo/GAZ_00067012">
        <rdf:type rdf:resource="http://purl.obolibrary.org/obo/ENVO_00000856"/>
        <obo:RO_0001025 rdf:resource="http://purl.obolibrary.org/obo/GAZ_00056201"/>
        <obo:IAO_0000115>A municipality in the Masaya Department of Nicaragua.</obo:IAO_0000115>
        <oboInOwl:hasOBONamespace>GAZ</oboInOwl:hasOBONamespace>
        <oboInOwl:id>GAZ:00067012</oboInOwl:id>
        <rdfs:label>Municipality of Masaya</rdfs:label>
    </owl:NamedIndividual>
    


    <!-- http://purl.obolibrary.org/obo/GAZ_00067013 -->

    <owl:NamedIndividual rdf:about="http://purl.obolibrary.org/obo/GAZ_00067013">
        <rdf:type rdf:resource="http://purl.obolibrary.org/obo/ENVO_00000856"/>
        <obo:RO_0001025 rdf:resource="http://purl.obolibrary.org/obo/GAZ_00056201"/>
        <obo:IAO_0000115>A municipality in the Masaya Department of Nicaragua.</obo:IAO_0000115>
        <oboInOwl:hasOBONamespace>GAZ</oboInOwl:hasOBONamespace>
        <oboInOwl:id>GAZ:00067013</oboInOwl:id>
        <rdfs:label>Municipality of La Concepcion</rdfs:label>
    </owl:NamedIndividual>
    


    <!-- http://purl.obolibrary.org/obo/GAZ_00067014 -->

    <owl:NamedIndividual rdf:about="http://purl.obolibrary.org/obo/GAZ_00067014">
        <rdf:type rdf:resource="http://purl.obolibrary.org/obo/ENVO_00000856"/>
        <obo:RO_0001025 rdf:resource="http://purl.obolibrary.org/obo/GAZ_00056201"/>
        <obo:IAO_0000115>A municipality in the Masaya Department of Nicaragua.</obo:IAO_0000115>
        <oboInOwl:hasOBONamespace>GAZ</oboInOwl:hasOBONamespace>
        <oboInOwl:id>GAZ:00067014</oboInOwl:id>
        <rdfs:label>Municipality of Niquinomo</rdfs:label>
    </owl:NamedIndividual>
    


    <!-- http://purl.obolibrary.org/obo/GAZ_00067015 -->

    <owl:NamedIndividual rdf:about="http://purl.obolibrary.org/obo/GAZ_00067015">
        <rdf:type rdf:resource="http://purl.obolibrary.org/obo/ENVO_00000856"/>
        <obo:RO_0001025 rdf:resource="http://purl.obolibrary.org/obo/GAZ_00056201"/>
        <obo:IAO_0000115>A municipality in the Masaya Department of Nicaragua.</obo:IAO_0000115>
        <oboInOwl:hasOBONamespace>GAZ</oboInOwl:hasOBONamespace>
        <oboInOwl:id>GAZ:00067015</oboInOwl:id>
        <rdfs:label>Municipality of Catarina</rdfs:label>
    </owl:NamedIndividual>
    


    <!-- http://purl.obolibrary.org/obo/GAZ_00067016 -->

    <owl:NamedIndividual rdf:about="http://purl.obolibrary.org/obo/GAZ_00067016">
        <rdf:type rdf:resource="http://purl.obolibrary.org/obo/ENVO_00000856"/>
        <obo:RO_0001025 rdf:resource="http://purl.obolibrary.org/obo/GAZ_00056201"/>
        <obo:IAO_0000115>A municipality in the Masaya Department of Nicaragua.</obo:IAO_0000115>
        <oboInOwl:hasOBONamespace>GAZ</oboInOwl:hasOBONamespace>
        <oboInOwl:id>GAZ:00067016</oboInOwl:id>
        <rdfs:label>Municipality of Nandasmo</rdfs:label>
    </owl:NamedIndividual>
    


    <!-- http://purl.obolibrary.org/obo/GAZ_00067017 -->

    <owl:NamedIndividual rdf:about="http://purl.obolibrary.org/obo/GAZ_00067017">
        <rdf:type rdf:resource="http://purl.obolibrary.org/obo/ENVO_00000856"/>
        <obo:RO_0001025 rdf:resource="http://purl.obolibrary.org/obo/GAZ_00066800"/>
        <obo:IAO_0000115>A municipality in the Matagalpa Department of Nicaragua.</obo:IAO_0000115>
        <oboInOwl:hasOBONamespace>GAZ</oboInOwl:hasOBONamespace>
        <oboInOwl:id>GAZ:00067017</oboInOwl:id>
        <rdfs:label>Municipality of Rio Blanco</rdfs:label>
    </owl:NamedIndividual>
    


    <!-- http://purl.obolibrary.org/obo/GAZ_00067018 -->

    <owl:NamedIndividual rdf:about="http://purl.obolibrary.org/obo/GAZ_00067018">
        <rdf:type rdf:resource="http://purl.obolibrary.org/obo/ENVO_00000856"/>
        <obo:RO_0001025 rdf:resource="http://purl.obolibrary.org/obo/GAZ_00066800"/>
        <obo:IAO_0000115>A municipality in the Matagalpa Department of Nicaragua.</obo:IAO_0000115>
        <oboInOwl:hasOBONamespace>GAZ</oboInOwl:hasOBONamespace>
        <oboInOwl:id>GAZ:00067018</oboInOwl:id>
        <rdfs:label>Municipality of San Ramon</rdfs:label>
    </owl:NamedIndividual>
    


    <!-- http://purl.obolibrary.org/obo/GAZ_00067019 -->

    <owl:NamedIndividual rdf:about="http://purl.obolibrary.org/obo/GAZ_00067019">
        <rdf:type rdf:resource="http://purl.obolibrary.org/obo/ENVO_00000856"/>
        <obo:RO_0001025 rdf:resource="http://purl.obolibrary.org/obo/GAZ_00066800"/>
        <obo:IAO_0000115>A municipality in the Matagalpa Department of Nicaragua.</obo:IAO_0000115>
        <oboInOwl:hasOBONamespace>GAZ</oboInOwl:hasOBONamespace>
        <oboInOwl:id>GAZ:00067019</oboInOwl:id>
        <rdfs:label>Municipality of Tuma-La Dalia</rdfs:label>
    </owl:NamedIndividual>
    


    <!-- http://purl.obolibrary.org/obo/GAZ_00067020 -->

    <owl:NamedIndividual rdf:about="http://purl.obolibrary.org/obo/GAZ_00067020">
        <rdf:type rdf:resource="http://purl.obolibrary.org/obo/ENVO_00000856"/>
        <obo:RO_0001025 rdf:resource="http://purl.obolibrary.org/obo/GAZ_00066800"/>
        <obo:IAO_0000115>A municipality in the Matagalpa Department of Nicaragua.</obo:IAO_0000115>
        <oboInOwl:hasOBONamespace>GAZ</oboInOwl:hasOBONamespace>
        <oboInOwl:id>GAZ:00067020</oboInOwl:id>
        <rdfs:label>Municipality of Sebaco</rdfs:label>
    </owl:NamedIndividual>
    


    <!-- http://purl.obolibrary.org/obo/GAZ_00067021 -->

    <owl:NamedIndividual rdf:about="http://purl.obolibrary.org/obo/GAZ_00067021">
        <rdf:type rdf:resource="http://purl.obolibrary.org/obo/ENVO_00000856"/>
        <obo:RO_0001025 rdf:resource="http://purl.obolibrary.org/obo/GAZ_00066800"/>
        <obo:IAO_0000115>A municipality in the Matagalpa Department of Nicaragua.</obo:IAO_0000115>
        <oboInOwl:hasOBONamespace>GAZ</oboInOwl:hasOBONamespace>
        <oboInOwl:id>GAZ:00067021</oboInOwl:id>
        <rdfs:label>Municipality of Esquipulas</rdfs:label>
    </owl:NamedIndividual>
    


    <!-- http://purl.obolibrary.org/obo/GAZ_00067022 -->

    <owl:NamedIndividual rdf:about="http://purl.obolibrary.org/obo/GAZ_00067022">
        <rdf:type rdf:resource="http://purl.obolibrary.org/obo/ENVO_00000856"/>
        <obo:RO_0001025 rdf:resource="http://purl.obolibrary.org/obo/GAZ_00066800"/>
        <obo:IAO_0000115>A municipality in the Matagalpa Department of Nicaragua.</obo:IAO_0000115>
        <oboInOwl:hasOBONamespace>GAZ</oboInOwl:hasOBONamespace>
        <oboInOwl:id>GAZ:00067022</oboInOwl:id>
        <rdfs:label>Municipality of Rancho Grande</rdfs:label>
    </owl:NamedIndividual>
    


    <!-- http://purl.obolibrary.org/obo/GAZ_00067023 -->

    <owl:NamedIndividual rdf:about="http://purl.obolibrary.org/obo/GAZ_00067023">
        <rdf:type rdf:resource="http://purl.obolibrary.org/obo/ENVO_00000856"/>
        <obo:RO_0001025 rdf:resource="http://purl.obolibrary.org/obo/GAZ_00066800"/>
        <obo:IAO_0000115>A municipality in the Matagalpa Department of Nicaragua.</obo:IAO_0000115>
        <oboInOwl:hasOBONamespace>GAZ</oboInOwl:hasOBONamespace>
        <oboInOwl:id>GAZ:00067023</oboInOwl:id>
        <rdfs:label>Municipality of Ciudad Dario</rdfs:label>
    </owl:NamedIndividual>
    


    <!-- http://purl.obolibrary.org/obo/GAZ_00067024 -->

    <owl:NamedIndividual rdf:about="http://purl.obolibrary.org/obo/GAZ_00067024">
        <rdf:type rdf:resource="http://purl.obolibrary.org/obo/ENVO_00000856"/>
        <obo:RO_0001025 rdf:resource="http://purl.obolibrary.org/obo/GAZ_00066800"/>
        <obo:IAO_0000115>A municipality in the Matagalpa Department of Nicaragua.</obo:IAO_0000115>
        <oboInOwl:hasOBONamespace>GAZ</oboInOwl:hasOBONamespace>
        <oboInOwl:id>GAZ:00067024</oboInOwl:id>
        <rdfs:label>Municipality of San Dionisio</rdfs:label>
    </owl:NamedIndividual>
    


    <!-- http://purl.obolibrary.org/obo/GAZ_00067025 -->

    <owl:NamedIndividual rdf:about="http://purl.obolibrary.org/obo/GAZ_00067025">
        <rdf:type rdf:resource="http://purl.obolibrary.org/obo/ENVO_00000856"/>
        <obo:RO_0001025 rdf:resource="http://purl.obolibrary.org/obo/GAZ_00066800"/>
        <obo:IAO_0000115>A municipality in the Matagalpa Department of Nicaragua.</obo:IAO_0000115>
        <oboInOwl:hasOBONamespace>GAZ</oboInOwl:hasOBONamespace>
        <oboInOwl:id>GAZ:00067025</oboInOwl:id>
        <rdfs:label>Municipality of Terrabona</rdfs:label>
    </owl:NamedIndividual>
    


    <!-- http://purl.obolibrary.org/obo/GAZ_00067026 -->

    <owl:NamedIndividual rdf:about="http://purl.obolibrary.org/obo/GAZ_00067026">
        <rdf:type rdf:resource="http://purl.obolibrary.org/obo/ENVO_00000856"/>
        <obo:RO_0001025 rdf:resource="http://purl.obolibrary.org/obo/GAZ_00066800"/>
        <obo:IAO_0000115>A municipality in the Matagalpa Department of Nicaragua.</obo:IAO_0000115>
        <oboInOwl:hasOBONamespace>GAZ</oboInOwl:hasOBONamespace>
        <oboInOwl:id>GAZ:00067026</oboInOwl:id>
        <rdfs:label>Municipality of Matiguas</rdfs:label>
    </owl:NamedIndividual>
    


    <!-- http://purl.obolibrary.org/obo/GAZ_00067027 -->

    <owl:NamedIndividual rdf:about="http://purl.obolibrary.org/obo/GAZ_00067027">
        <rdf:type rdf:resource="http://purl.obolibrary.org/obo/ENVO_00000856"/>
        <obo:RO_0001025 rdf:resource="http://purl.obolibrary.org/obo/GAZ_00066800"/>
        <obo:IAO_0000115>A municipality in the Matagalpa Department of Nicaragua.</obo:IAO_0000115>
        <oboInOwl:hasOBONamespace>GAZ</oboInOwl:hasOBONamespace>
        <oboInOwl:id>GAZ:00067027</oboInOwl:id>
        <rdfs:label>Municipality of Muy Muy</rdfs:label>
    </owl:NamedIndividual>
    


    <!-- http://purl.obolibrary.org/obo/GAZ_00067028 -->

    <owl:NamedIndividual rdf:about="http://purl.obolibrary.org/obo/GAZ_00067028">
        <rdf:type rdf:resource="http://purl.obolibrary.org/obo/ENVO_00000856"/>
        <obo:RO_0001025 rdf:resource="http://purl.obolibrary.org/obo/GAZ_00066800"/>
        <obo:IAO_0000115>A municipality in the Matagalpa Department of Nicaragua.</obo:IAO_0000115>
        <oboInOwl:hasOBONamespace>GAZ</oboInOwl:hasOBONamespace>
        <oboInOwl:id>GAZ:00067028</oboInOwl:id>
        <rdfs:label>Municipality of San Isidro</rdfs:label>
    </owl:NamedIndividual>
    


    <!-- http://purl.obolibrary.org/obo/GAZ_00067029 -->

    <owl:NamedIndividual rdf:about="http://purl.obolibrary.org/obo/GAZ_00067029">
        <rdf:type rdf:resource="http://purl.obolibrary.org/obo/ENVO_00000856"/>
        <obo:RO_0001025 rdf:resource="http://purl.obolibrary.org/obo/GAZ_00066800"/>
        <obo:IAO_0000115>A municipality in the Matagalpa Department of Nicaragua.</obo:IAO_0000115>
        <oboInOwl:hasOBONamespace>GAZ</oboInOwl:hasOBONamespace>
        <oboInOwl:id>GAZ:00067029</oboInOwl:id>
        <rdfs:label>Municipality of Matagalpa</rdfs:label>
    </owl:NamedIndividual>
    


    <!-- http://purl.obolibrary.org/obo/GAZ_00067030 -->

    <owl:NamedIndividual rdf:about="http://purl.obolibrary.org/obo/GAZ_00067030">
        <rdf:type rdf:resource="http://purl.obolibrary.org/obo/ENVO_00000856"/>
        <obo:RO_0001025 rdf:resource="http://purl.obolibrary.org/obo/GAZ_00066802"/>
        <obo:IAO_0000115>A municipality in the Nueva Segovia Department of Nicaragua.</obo:IAO_0000115>
        <oboInOwl:hasOBONamespace>GAZ</oboInOwl:hasOBONamespace>
        <oboInOwl:id>GAZ:00067030</oboInOwl:id>
        <rdfs:label>Municipality of Dipilto</rdfs:label>
    </owl:NamedIndividual>
    


    <!-- http://purl.obolibrary.org/obo/GAZ_00067031 -->

    <owl:NamedIndividual rdf:about="http://purl.obolibrary.org/obo/GAZ_00067031">
        <rdf:type rdf:resource="http://purl.obolibrary.org/obo/ENVO_00000856"/>
        <obo:RO_0001025 rdf:resource="http://purl.obolibrary.org/obo/GAZ_00066802"/>
        <obo:IAO_0000115>A municipality in the Nueva Segovia Department of Nicaragua.</obo:IAO_0000115>
        <oboInOwl:hasOBONamespace>GAZ</oboInOwl:hasOBONamespace>
        <oboInOwl:id>GAZ:00067031</oboInOwl:id>
        <rdfs:label>Municipality of Quilali</rdfs:label>
    </owl:NamedIndividual>
    


    <!-- http://purl.obolibrary.org/obo/GAZ_00067032 -->

    <owl:NamedIndividual rdf:about="http://purl.obolibrary.org/obo/GAZ_00067032">
        <rdf:type rdf:resource="http://purl.obolibrary.org/obo/ENVO_00000856"/>
        <obo:RO_0001025 rdf:resource="http://purl.obolibrary.org/obo/GAZ_00066802"/>
        <obo:IAO_0000115>A municipality in the Nueva Segovia Department of Nicaragua.</obo:IAO_0000115>
        <oboInOwl:hasOBONamespace>GAZ</oboInOwl:hasOBONamespace>
        <oboInOwl:id>GAZ:00067032</oboInOwl:id>
        <rdfs:label>Municipality of Wiwili de Nueva Segovia</rdfs:label>
    </owl:NamedIndividual>
    


    <!-- http://purl.obolibrary.org/obo/GAZ_00067033 -->

    <owl:NamedIndividual rdf:about="http://purl.obolibrary.org/obo/GAZ_00067033">
        <rdf:type rdf:resource="http://purl.obolibrary.org/obo/ENVO_00000856"/>
        <obo:RO_0001025 rdf:resource="http://purl.obolibrary.org/obo/GAZ_00066802"/>
        <obo:IAO_0000115>A municipality in the Nueva Segovia Department of Nicaragua.</obo:IAO_0000115>
        <oboInOwl:hasOBONamespace>GAZ</oboInOwl:hasOBONamespace>
        <oboInOwl:id>GAZ:00067033</oboInOwl:id>
        <rdfs:label>Municipality of Santa Maria</rdfs:label>
    </owl:NamedIndividual>
    


    <!-- http://purl.obolibrary.org/obo/GAZ_00067034 -->

    <owl:NamedIndividual rdf:about="http://purl.obolibrary.org/obo/GAZ_00067034">
        <rdf:type rdf:resource="http://purl.obolibrary.org/obo/ENVO_00000856"/>
        <obo:RO_0001025 rdf:resource="http://purl.obolibrary.org/obo/GAZ_00066802"/>
        <obo:IAO_0000115>A municipality in the Nueva Segovia Department of Nicaragua.</obo:IAO_0000115>
        <oboInOwl:hasOBONamespace>GAZ</oboInOwl:hasOBONamespace>
        <oboInOwl:id>GAZ:00067034</oboInOwl:id>
        <rdfs:label>Municipality of El Jicaro</rdfs:label>
    </owl:NamedIndividual>
    


    <!-- http://purl.obolibrary.org/obo/GAZ_00067035 -->

    <owl:NamedIndividual rdf:about="http://purl.obolibrary.org/obo/GAZ_00067035">
        <rdf:type rdf:resource="http://purl.obolibrary.org/obo/ENVO_00000856"/>
        <obo:RO_0001025 rdf:resource="http://purl.obolibrary.org/obo/GAZ_00066802"/>
        <obo:IAO_0000115>A municipality in the Nueva Segovia Department of Nicaragua.</obo:IAO_0000115>
        <oboInOwl:hasOBONamespace>GAZ</oboInOwl:hasOBONamespace>
        <oboInOwl:id>GAZ:00067035</oboInOwl:id>
        <rdfs:label>Municipality of Jalapa</rdfs:label>
    </owl:NamedIndividual>
    


    <!-- http://purl.obolibrary.org/obo/GAZ_00067036 -->

    <owl:NamedIndividual rdf:about="http://purl.obolibrary.org/obo/GAZ_00067036">
        <rdf:type rdf:resource="http://purl.obolibrary.org/obo/ENVO_00000856"/>
        <obo:RO_0001025 rdf:resource="http://purl.obolibrary.org/obo/GAZ_00066802"/>
        <obo:IAO_0000115>A municipality in the Nueva Segovia Department of Nicaragua.</obo:IAO_0000115>
        <oboInOwl:hasOBONamespace>GAZ</oboInOwl:hasOBONamespace>
        <oboInOwl:id>GAZ:00067036</oboInOwl:id>
        <rdfs:label>Municipality of Mozonte</rdfs:label>
    </owl:NamedIndividual>
    


    <!-- http://purl.obolibrary.org/obo/GAZ_00067037 -->

    <owl:NamedIndividual rdf:about="http://purl.obolibrary.org/obo/GAZ_00067037">
        <rdf:type rdf:resource="http://purl.obolibrary.org/obo/ENVO_00000856"/>
        <obo:RO_0001025 rdf:resource="http://purl.obolibrary.org/obo/GAZ_00066802"/>
        <obo:IAO_0000115>A municipality in the Nueva Segovia Department of Nicaragua.</obo:IAO_0000115>
        <oboInOwl:hasOBONamespace>GAZ</oboInOwl:hasOBONamespace>
        <oboInOwl:id>GAZ:00067037</oboInOwl:id>
        <rdfs:label>Municipality of San Fernando</rdfs:label>
    </owl:NamedIndividual>
    


    <!-- http://purl.obolibrary.org/obo/GAZ_00067038 -->

    <owl:NamedIndividual rdf:about="http://purl.obolibrary.org/obo/GAZ_00067038">
        <rdf:type rdf:resource="http://purl.obolibrary.org/obo/ENVO_00000856"/>
        <obo:RO_0001025 rdf:resource="http://purl.obolibrary.org/obo/GAZ_00066802"/>
        <obo:IAO_0000115>A municipality in the Nueva Segovia Department of Nicaragua.</obo:IAO_0000115>
        <oboInOwl:hasOBONamespace>GAZ</oboInOwl:hasOBONamespace>
        <oboInOwl:id>GAZ:00067038</oboInOwl:id>
        <rdfs:label>Municipality of Ocotal</rdfs:label>
    </owl:NamedIndividual>
    


    <!-- http://purl.obolibrary.org/obo/GAZ_00067039 -->

    <owl:NamedIndividual rdf:about="http://purl.obolibrary.org/obo/GAZ_00067039">
        <rdf:type rdf:resource="http://purl.obolibrary.org/obo/ENVO_00000856"/>
        <obo:RO_0001025 rdf:resource="http://purl.obolibrary.org/obo/GAZ_00066802"/>
        <obo:IAO_0000115>A municipality in the Nueva Segovia Department of Nicaragua.</obo:IAO_0000115>
        <oboInOwl:hasOBONamespace>GAZ</oboInOwl:hasOBONamespace>
        <oboInOwl:id>GAZ:00067039</oboInOwl:id>
        <rdfs:label>Municipality of Macuelizo</rdfs:label>
    </owl:NamedIndividual>
    


    <!-- http://purl.obolibrary.org/obo/GAZ_00067040 -->

    <owl:NamedIndividual rdf:about="http://purl.obolibrary.org/obo/GAZ_00067040">
        <rdf:type rdf:resource="http://purl.obolibrary.org/obo/ENVO_00000856"/>
        <obo:RO_0001025 rdf:resource="http://purl.obolibrary.org/obo/GAZ_00066802"/>
        <obo:IAO_0000115>A municipality in the Nueva Segovia Department of Nicaragua.</obo:IAO_0000115>
        <oboInOwl:hasOBONamespace>GAZ</oboInOwl:hasOBONamespace>
        <oboInOwl:id>GAZ:00067040</oboInOwl:id>
        <rdfs:label>Municipality of Murra</rdfs:label>
    </owl:NamedIndividual>
    


    <!-- http://purl.obolibrary.org/obo/GAZ_00067041 -->

    <owl:NamedIndividual rdf:about="http://purl.obolibrary.org/obo/GAZ_00067041">
        <rdf:type rdf:resource="http://purl.obolibrary.org/obo/ENVO_00000856"/>
        <obo:RO_0001025 rdf:resource="http://purl.obolibrary.org/obo/GAZ_00066802"/>
        <obo:IAO_0000115>A municipality in the Nueva Segovia Department of Nicaragua.</obo:IAO_0000115>
        <oboInOwl:hasOBONamespace>GAZ</oboInOwl:hasOBONamespace>
        <oboInOwl:id>GAZ:00067041</oboInOwl:id>
        <rdfs:label>Municipality of Ciudad Antigua</rdfs:label>
    </owl:NamedIndividual>
    


    <!-- http://purl.obolibrary.org/obo/GAZ_00067042 -->

    <owl:NamedIndividual rdf:about="http://purl.obolibrary.org/obo/GAZ_00067042">
        <rdf:type rdf:resource="http://purl.obolibrary.org/obo/ENVO_00000856"/>
        <obo:RO_0001025 rdf:resource="http://purl.obolibrary.org/obo/GAZ_00056208"/>
        <obo:IAO_0000115>A municipality in the Rivas Department of Nicaragua.</obo:IAO_0000115>
        <oboInOwl:hasOBONamespace>GAZ</oboInOwl:hasOBONamespace>
        <oboInOwl:id>GAZ:00067042</oboInOwl:id>
        <rdfs:label>Municipality of San Juan del Sur</rdfs:label>
    </owl:NamedIndividual>
    


    <!-- http://purl.obolibrary.org/obo/GAZ_00067043 -->

    <owl:NamedIndividual rdf:about="http://purl.obolibrary.org/obo/GAZ_00067043">
        <rdf:type rdf:resource="http://purl.obolibrary.org/obo/ENVO_00000856"/>
        <obo:RO_0001025 rdf:resource="http://purl.obolibrary.org/obo/GAZ_00056208"/>
        <obo:IAO_0000115>A municipality in the Rivas Department of Nicaragua.</obo:IAO_0000115>
        <oboInOwl:hasOBONamespace>GAZ</oboInOwl:hasOBONamespace>
        <oboInOwl:id>GAZ:00067043</oboInOwl:id>
        <rdfs:label>Municipality of Tola</rdfs:label>
    </owl:NamedIndividual>
    


    <!-- http://purl.obolibrary.org/obo/GAZ_00067044 -->

    <owl:NamedIndividual rdf:about="http://purl.obolibrary.org/obo/GAZ_00067044">
        <rdf:type rdf:resource="http://purl.obolibrary.org/obo/ENVO_00000856"/>
        <obo:RO_0001025 rdf:resource="http://purl.obolibrary.org/obo/GAZ_00056208"/>
        <obo:IAO_0000115>A municipality in the Rivas Department of Nicaragua.</obo:IAO_0000115>
        <oboInOwl:hasOBONamespace>GAZ</oboInOwl:hasOBONamespace>
        <oboInOwl:id>GAZ:00067044</oboInOwl:id>
        <rdfs:label>Municipality of Belen</rdfs:label>
    </owl:NamedIndividual>
    


    <!-- http://purl.obolibrary.org/obo/GAZ_00067045 -->

    <owl:NamedIndividual rdf:about="http://purl.obolibrary.org/obo/GAZ_00067045">
        <rdf:type rdf:resource="http://purl.obolibrary.org/obo/ENVO_00000856"/>
        <obo:RO_0001025 rdf:resource="http://purl.obolibrary.org/obo/GAZ_00056208"/>
        <obo:IAO_0000115>A municipality in the Rivas Department of Nicaragua.</obo:IAO_0000115>
        <oboInOwl:hasOBONamespace>GAZ</oboInOwl:hasOBONamespace>
        <oboInOwl:id>GAZ:00067045</oboInOwl:id>
        <rdfs:label>Municipality of Rivas</rdfs:label>
    </owl:NamedIndividual>
    


    <!-- http://purl.obolibrary.org/obo/GAZ_00067046 -->

    <owl:NamedIndividual rdf:about="http://purl.obolibrary.org/obo/GAZ_00067046">
        <rdf:type rdf:resource="http://purl.obolibrary.org/obo/ENVO_00000856"/>
        <obo:RO_0001025 rdf:resource="http://purl.obolibrary.org/obo/GAZ_00056208"/>
        <obo:IAO_0000115>A municipality in the Rivas Department of Nicaragua.</obo:IAO_0000115>
        <oboInOwl:hasOBONamespace>GAZ</oboInOwl:hasOBONamespace>
        <oboInOwl:id>GAZ:00067046</oboInOwl:id>
        <rdfs:label>Municipality of Potosi</rdfs:label>
    </owl:NamedIndividual>
    


    <!-- http://purl.obolibrary.org/obo/GAZ_00067047 -->

    <owl:NamedIndividual rdf:about="http://purl.obolibrary.org/obo/GAZ_00067047">
        <rdf:type rdf:resource="http://purl.obolibrary.org/obo/ENVO_00000856"/>
        <obo:RO_0001025 rdf:resource="http://purl.obolibrary.org/obo/GAZ_00056208"/>
        <obo:IAO_0000115>A municipality in the Rivas Department of Nicaragua.</obo:IAO_0000115>
        <oboInOwl:hasOBONamespace>GAZ</oboInOwl:hasOBONamespace>
        <oboInOwl:id>GAZ:00067047</oboInOwl:id>
        <rdfs:label>Municipality of Buenos Aires</rdfs:label>
    </owl:NamedIndividual>
    


    <!-- http://purl.obolibrary.org/obo/GAZ_00067048 -->

    <owl:NamedIndividual rdf:about="http://purl.obolibrary.org/obo/GAZ_00067048">
        <rdf:type rdf:resource="http://purl.obolibrary.org/obo/ENVO_00000856"/>
        <obo:RO_0001025 rdf:resource="http://purl.obolibrary.org/obo/GAZ_00056208"/>
        <obo:IAO_0000115>A municipality in the Rivas Department of Nicaragua.</obo:IAO_0000115>
        <oboInOwl:hasOBONamespace>GAZ</oboInOwl:hasOBONamespace>
        <oboInOwl:id>GAZ:00067048</oboInOwl:id>
        <rdfs:label>Municipality of San Jorge</rdfs:label>
    </owl:NamedIndividual>
    


    <!-- http://purl.obolibrary.org/obo/GAZ_00067049 -->

    <owl:NamedIndividual rdf:about="http://purl.obolibrary.org/obo/GAZ_00067049">
        <rdf:type rdf:resource="http://purl.obolibrary.org/obo/ENVO_00000856"/>
        <obo:RO_0001025 rdf:resource="http://purl.obolibrary.org/obo/GAZ_00056208"/>
        <obo:IAO_0000115>A municipality in the Rivas Department of Nicaragua.</obo:IAO_0000115>
        <oboInOwl:hasOBONamespace>GAZ</oboInOwl:hasOBONamespace>
        <oboInOwl:id>GAZ:00067049</oboInOwl:id>
        <rdfs:label>Municipality of Cardenas</rdfs:label>
    </owl:NamedIndividual>
    


    <!-- http://purl.obolibrary.org/obo/GAZ_00067050 -->

    <owl:NamedIndividual rdf:about="http://purl.obolibrary.org/obo/GAZ_00067050">
        <rdf:type rdf:resource="http://purl.obolibrary.org/obo/ENVO_00000856"/>
        <obo:RO_0001025 rdf:resource="http://purl.obolibrary.org/obo/GAZ_00047257"/>
        <obo:IAO_0000115>A municipality in the Rivas Department of Nicaragua.</obo:IAO_0000115>
        <oboInOwl:hasOBONamespace>GAZ</oboInOwl:hasOBONamespace>
        <oboInOwl:id>GAZ:00067050</oboInOwl:id>
        <rdfs:label>Municipality of Moyogalpa</rdfs:label>
    </owl:NamedIndividual>
    


    <!-- http://purl.obolibrary.org/obo/GAZ_00067051 -->

    <owl:NamedIndividual rdf:about="http://purl.obolibrary.org/obo/GAZ_00067051">
        <rdf:type rdf:resource="http://purl.obolibrary.org/obo/ENVO_00000856"/>
        <obo:RO_0001025 rdf:resource="http://purl.obolibrary.org/obo/GAZ_00047257"/>
        <obo:IAO_0000115>A municipality in the Rivas Department of Nicaragua.</obo:IAO_0000115>
        <oboInOwl:hasOBONamespace>GAZ</oboInOwl:hasOBONamespace>
        <oboInOwl:id>GAZ:00067051</oboInOwl:id>
        <rdfs:label>Municipality of Altagracia</rdfs:label>
    </owl:NamedIndividual>
    


    <!-- http://purl.obolibrary.org/obo/GAZ_00067052 -->

    <owl:NamedIndividual rdf:about="http://purl.obolibrary.org/obo/GAZ_00067052">
        <rdf:type rdf:resource="http://purl.obolibrary.org/obo/ENVO_00000856"/>
        <obo:RO_0001025 rdf:resource="http://purl.obolibrary.org/obo/GAZ_00047261"/>
        <obo:IAO_0000115>A municipality in the Rio San Juan Department of Nicaragua.</obo:IAO_0000115>
        <oboInOwl:hasOBONamespace>GAZ</oboInOwl:hasOBONamespace>
        <oboInOwl:id>GAZ:00067052</oboInOwl:id>
        <rdfs:label>Municipality of San Juan del Norte</rdfs:label>
    </owl:NamedIndividual>
    


    <!-- http://purl.obolibrary.org/obo/GAZ_00067053 -->

    <owl:NamedIndividual rdf:about="http://purl.obolibrary.org/obo/GAZ_00067053">
        <rdf:type rdf:resource="http://purl.obolibrary.org/obo/ENVO_00000856"/>
        <obo:RO_0001025 rdf:resource="http://purl.obolibrary.org/obo/GAZ_00047261"/>
        <obo:IAO_0000115>A municipality in the Rio San Juan Department of Nicaragua.</obo:IAO_0000115>
        <oboInOwl:hasOBONamespace>GAZ</oboInOwl:hasOBONamespace>
        <oboInOwl:id>GAZ:00067053</oboInOwl:id>
        <rdfs:label>Municipality of San Miguelito</rdfs:label>
    </owl:NamedIndividual>
    


    <!-- http://purl.obolibrary.org/obo/GAZ_00067054 -->

    <owl:NamedIndividual rdf:about="http://purl.obolibrary.org/obo/GAZ_00067054">
        <rdf:type rdf:resource="http://purl.obolibrary.org/obo/ENVO_00000856"/>
        <obo:RO_0001025 rdf:resource="http://purl.obolibrary.org/obo/GAZ_00047261"/>
        <obo:IAO_0000115>A municipality in the Rio San Juan Department of Nicaragua.</obo:IAO_0000115>
        <oboInOwl:hasOBONamespace>GAZ</oboInOwl:hasOBONamespace>
        <oboInOwl:id>GAZ:00067054</oboInOwl:id>
        <rdfs:label>Municipality of El Castillo</rdfs:label>
    </owl:NamedIndividual>
    


    <!-- http://purl.obolibrary.org/obo/GAZ_00067055 -->

    <owl:NamedIndividual rdf:about="http://purl.obolibrary.org/obo/GAZ_00067055">
        <rdf:type rdf:resource="http://purl.obolibrary.org/obo/ENVO_00000856"/>
        <obo:RO_0001025 rdf:resource="http://purl.obolibrary.org/obo/GAZ_00047261"/>
        <obo:IAO_0000115>A municipality in the Rio San Juan Department of Nicaragua.</obo:IAO_0000115>
        <oboInOwl:hasOBONamespace>GAZ</oboInOwl:hasOBONamespace>
        <oboInOwl:id>GAZ:00067055</oboInOwl:id>
        <rdfs:label>Municipality of El Almendro</rdfs:label>
    </owl:NamedIndividual>
    


    <!-- http://purl.obolibrary.org/obo/GAZ_00067056 -->

    <owl:NamedIndividual rdf:about="http://purl.obolibrary.org/obo/GAZ_00067056">
        <rdf:type rdf:resource="http://purl.obolibrary.org/obo/ENVO_00000856"/>
        <obo:RO_0001025 rdf:resource="http://purl.obolibrary.org/obo/GAZ_00047261"/>
        <obo:IAO_0000115>A municipality in the Rio San Juan Department of Nicaragua.</obo:IAO_0000115>
        <oboInOwl:hasOBONamespace>GAZ</oboInOwl:hasOBONamespace>
        <oboInOwl:id>GAZ:00067056</oboInOwl:id>
        <rdfs:label>Municipality of San Carlos</rdfs:label>
    </owl:NamedIndividual>
    


    <!-- http://purl.obolibrary.org/obo/GAZ_00067057 -->

    <owl:NamedIndividual rdf:about="http://purl.obolibrary.org/obo/GAZ_00067057">
        <rdf:type rdf:resource="http://purl.obolibrary.org/obo/ENVO_00000856"/>
        <obo:RO_0001025 rdf:resource="http://purl.obolibrary.org/obo/GAZ_00047261"/>
        <obo:IAO_0000115>A municipality in the Rio San Juan Department of Nicaragua.</obo:IAO_0000115>
        <oboInOwl:hasOBONamespace>GAZ</oboInOwl:hasOBONamespace>
        <oboInOwl:id>GAZ:00067057</oboInOwl:id>
        <rdfs:label>Municipality of Morrito</rdfs:label>
    </owl:NamedIndividual>
    


    <!-- http://purl.obolibrary.org/obo/GAZ_00067058 -->

    <owl:NamedIndividual rdf:about="http://purl.obolibrary.org/obo/GAZ_00067058">
        <rdf:type rdf:resource="http://purl.obolibrary.org/obo/ENVO_00000856"/>
        <obo:RO_0001025 rdf:resource="http://purl.obolibrary.org/obo/GAZ_00047244"/>
        <obo:IAO_0000115>A municipality in the Region Autonoma del Atlantico Norte department of Nicaragua.</obo:IAO_0000115>
        <oboInOwl:hasOBONamespace>GAZ</oboInOwl:hasOBONamespace>
        <oboInOwl:id>GAZ:00067058</oboInOwl:id>
        <rdfs:label>Municipality of Waslala</rdfs:label>
    </owl:NamedIndividual>
    


    <!-- http://purl.obolibrary.org/obo/GAZ_00067059 -->

    <owl:NamedIndividual rdf:about="http://purl.obolibrary.org/obo/GAZ_00067059">
        <rdf:type rdf:resource="http://purl.obolibrary.org/obo/ENVO_00000856"/>
        <obo:RO_0001025 rdf:resource="http://purl.obolibrary.org/obo/GAZ_00047244"/>
        <obo:IAO_0000115>A municipality in the Region Autonoma del Atlantico Norte department of Nicaragua.</obo:IAO_0000115>
        <oboInOwl:hasOBONamespace>GAZ</oboInOwl:hasOBONamespace>
        <oboInOwl:id>GAZ:00067059</oboInOwl:id>
        <rdfs:label>Municipality of Mulukuku</rdfs:label>
    </owl:NamedIndividual>
    


    <!-- http://purl.obolibrary.org/obo/GAZ_00067060 -->

    <owl:NamedIndividual rdf:about="http://purl.obolibrary.org/obo/GAZ_00067060">
        <rdf:type rdf:resource="http://purl.obolibrary.org/obo/ENVO_00000856"/>
        <obo:RO_0001025 rdf:resource="http://purl.obolibrary.org/obo/GAZ_00047244"/>
        <obo:IAO_0000115>A municipality in the Region Autonoma del Atlantico Norte department of Nicaragua.</obo:IAO_0000115>
        <oboInOwl:hasOBONamespace>GAZ</oboInOwl:hasOBONamespace>
        <oboInOwl:id>GAZ:00067060</oboInOwl:id>
        <rdfs:label>Municipality of Siuna</rdfs:label>
    </owl:NamedIndividual>
    


    <!-- http://purl.obolibrary.org/obo/GAZ_00067061 -->

    <owl:NamedIndividual rdf:about="http://purl.obolibrary.org/obo/GAZ_00067061">
        <rdf:type rdf:resource="http://purl.obolibrary.org/obo/ENVO_00000856"/>
        <obo:RO_0001025 rdf:resource="http://purl.obolibrary.org/obo/GAZ_00047244"/>
        <obo:IAO_0000115>A municipality in the Region Autonoma del Atlantico Norte department of Nicaragua.</obo:IAO_0000115>
        <oboInOwl:hasOBONamespace>GAZ</oboInOwl:hasOBONamespace>
        <oboInOwl:id>GAZ:00067061</oboInOwl:id>
        <rdfs:label>Municipality of Puerto Cabezas</rdfs:label>
    </owl:NamedIndividual>
    


    <!-- http://purl.obolibrary.org/obo/GAZ_00067062 -->

    <owl:NamedIndividual rdf:about="http://purl.obolibrary.org/obo/GAZ_00067062">
        <rdf:type rdf:resource="http://purl.obolibrary.org/obo/ENVO_00000856"/>
        <obo:RO_0001025 rdf:resource="http://purl.obolibrary.org/obo/GAZ_00047244"/>
        <obo:IAO_0000115>A municipality in the Region Autonoma del Atlantico Norte department of Nicaragua.</obo:IAO_0000115>
        <oboInOwl:hasOBONamespace>GAZ</oboInOwl:hasOBONamespace>
        <oboInOwl:id>GAZ:00067062</oboInOwl:id>
        <rdfs:label>Municipality of Waspam</rdfs:label>
    </owl:NamedIndividual>
    


    <!-- http://purl.obolibrary.org/obo/GAZ_00067063 -->

    <owl:NamedIndividual rdf:about="http://purl.obolibrary.org/obo/GAZ_00067063">
        <rdf:type rdf:resource="http://purl.obolibrary.org/obo/ENVO_00000856"/>
        <obo:RO_0001025 rdf:resource="http://purl.obolibrary.org/obo/GAZ_00047244"/>
        <obo:IAO_0000115>A municipality in the Region Autonoma del Atlantico Norte department of Nicaragua.</obo:IAO_0000115>
        <oboInOwl:hasOBONamespace>GAZ</oboInOwl:hasOBONamespace>
        <oboInOwl:id>GAZ:00067063</oboInOwl:id>
        <rdfs:label>Municipality of Bonanza</rdfs:label>
    </owl:NamedIndividual>
    


    <!-- http://purl.obolibrary.org/obo/GAZ_00067064 -->

    <owl:NamedIndividual rdf:about="http://purl.obolibrary.org/obo/GAZ_00067064">
        <rdf:type rdf:resource="http://purl.obolibrary.org/obo/ENVO_00000856"/>
        <obo:RO_0001025 rdf:resource="http://purl.obolibrary.org/obo/GAZ_00047244"/>
        <obo:IAO_0000115>A municipality in the Region Autonoma del Atlantico Norte department of Nicaragua.</obo:IAO_0000115>
        <oboInOwl:hasOBONamespace>GAZ</oboInOwl:hasOBONamespace>
        <oboInOwl:id>GAZ:00067064</oboInOwl:id>
        <rdfs:label>Municipality of Prinzapolka</rdfs:label>
    </owl:NamedIndividual>
    


    <!-- http://purl.obolibrary.org/obo/GAZ_00067065 -->

    <owl:NamedIndividual rdf:about="http://purl.obolibrary.org/obo/GAZ_00067065">
        <rdf:type rdf:resource="http://purl.obolibrary.org/obo/ENVO_00000856"/>
        <obo:RO_0001025 rdf:resource="http://purl.obolibrary.org/obo/GAZ_00047244"/>
        <obo:IAO_0000115>A municipality in the Region Autonoma del Atlantico Norte department of Nicaragua.</obo:IAO_0000115>
        <oboInOwl:hasOBONamespace>GAZ</oboInOwl:hasOBONamespace>
        <oboInOwl:id>GAZ:00067065</oboInOwl:id>
        <rdfs:label>Municipality of Rosita</rdfs:label>
    </owl:NamedIndividual>
    


    <!-- http://purl.obolibrary.org/obo/GAZ_00067066 -->

    <owl:NamedIndividual rdf:about="http://purl.obolibrary.org/obo/GAZ_00067066">
        <rdf:type rdf:resource="http://purl.obolibrary.org/obo/ENVO_00000856"/>
        <obo:RO_0001025 rdf:resource="http://purl.obolibrary.org/obo/GAZ_00047243"/>
        <obo:IAO_0000115>A municipality in Region Autonoma del Atlantico Sur, Nicaragua.</obo:IAO_0000115>
        <oboInOwl:hasOBONamespace>GAZ</oboInOwl:hasOBONamespace>
        <oboInOwl:id>GAZ:00067066</oboInOwl:id>
        <rdfs:label>Municipality of La Cruz de Rio Grande</rdfs:label>
    </owl:NamedIndividual>
    


    <!-- http://purl.obolibrary.org/obo/GAZ_00067068 -->

    <owl:NamedIndividual rdf:about="http://purl.obolibrary.org/obo/GAZ_00067068">
        <rdf:type rdf:resource="http://purl.obolibrary.org/obo/ENVO_00000856"/>
        <obo:RO_0001025 rdf:resource="http://purl.obolibrary.org/obo/GAZ_00047243"/>
        <obo:IAO_0000115>A municipality in Region Autonoma del Atlantico Sur, Nicaragua.</obo:IAO_0000115>
        <oboInOwl:hasOBONamespace>GAZ</oboInOwl:hasOBONamespace>
        <oboInOwl:id>GAZ:00067068</oboInOwl:id>
        <rdfs:label>Municipality of Bocana de Paiwas</rdfs:label>
    </owl:NamedIndividual>
    


    <!-- http://purl.obolibrary.org/obo/GAZ_00067069 -->

    <owl:NamedIndividual rdf:about="http://purl.obolibrary.org/obo/GAZ_00067069">
        <rdf:type rdf:resource="http://purl.obolibrary.org/obo/ENVO_00000856"/>
        <obo:RO_0001025 rdf:resource="http://purl.obolibrary.org/obo/GAZ_00047243"/>
        <obo:IAO_0000115>A municipality in Region Autonoma del Atlantico Sur, Nicaragua. It is located on Bluefields Bay at the mouth of the Escondido River.</obo:IAO_0000115>
        <oboInOwl:hasOBONamespace>GAZ</oboInOwl:hasOBONamespace>
        <oboInOwl:id>GAZ:00067069</oboInOwl:id>
        <rdfs:label>Municipality of Bluefields</rdfs:label>
    </owl:NamedIndividual>
    


    <!-- http://purl.obolibrary.org/obo/GAZ_00067070 -->

    <owl:NamedIndividual rdf:about="http://purl.obolibrary.org/obo/GAZ_00067070">
        <rdf:type rdf:resource="http://purl.obolibrary.org/obo/ENVO_00000856"/>
        <obo:RO_0001025 rdf:resource="http://purl.obolibrary.org/obo/GAZ_00047243"/>
        <obo:IAO_0000115>A municipality in Region Autonoma del Atlantico Sur, Nicaragua.</obo:IAO_0000115>
        <oboInOwl:hasOBONamespace>GAZ</oboInOwl:hasOBONamespace>
        <oboInOwl:id>GAZ:00067070</oboInOwl:id>
        <rdfs:label>Municipality of Kukra Hill</rdfs:label>
    </owl:NamedIndividual>
    


    <!-- http://purl.obolibrary.org/obo/GAZ_00067071 -->

    <owl:NamedIndividual rdf:about="http://purl.obolibrary.org/obo/GAZ_00067071">
        <rdf:type rdf:resource="http://purl.obolibrary.org/obo/ENVO_00000856"/>
        <obo:RO_0001025 rdf:resource="http://purl.obolibrary.org/obo/GAZ_00047243"/>
        <obo:IAO_0000115>A municipality in Region Autonoma del Atlantico Sur, Nicaragua.</obo:IAO_0000115>
        <oboInOwl:hasOBONamespace>GAZ</oboInOwl:hasOBONamespace>
        <oboInOwl:id>GAZ:00067071</oboInOwl:id>
        <rdfs:label>Municipality of Muelle de los Bueyes</rdfs:label>
    </owl:NamedIndividual>
    


    <!-- http://purl.obolibrary.org/obo/GAZ_00067072 -->

    <owl:NamedIndividual rdf:about="http://purl.obolibrary.org/obo/GAZ_00067072">
        <rdf:type rdf:resource="http://purl.obolibrary.org/obo/ENVO_00000856"/>
        <obo:RO_0001025 rdf:resource="http://purl.obolibrary.org/obo/GAZ_00047243"/>
        <obo:IAO_0000115>A municipality in Region Autonoma del Atlantico Sur, Nicaragua.</obo:IAO_0000115>
        <oboInOwl:hasOBONamespace>GAZ</oboInOwl:hasOBONamespace>
        <oboInOwl:id>GAZ:00067072</oboInOwl:id>
        <rdfs:label>Municipality of Laguna de Perlas</rdfs:label>
    </owl:NamedIndividual>
    


    <!-- http://purl.obolibrary.org/obo/GAZ_00067073 -->

    <owl:NamedIndividual rdf:about="http://purl.obolibrary.org/obo/GAZ_00067073">
        <rdf:type rdf:resource="http://purl.obolibrary.org/obo/ENVO_00000856"/>
        <obo:RO_0001025 rdf:resource="http://purl.obolibrary.org/obo/GAZ_00047243"/>
        <obo:IAO_0000115>A municipality in Region Autonoma del Atlantico Sur, Nicaragua.</obo:IAO_0000115>
        <oboInOwl:hasOBONamespace>GAZ</oboInOwl:hasOBONamespace>
        <oboInOwl:id>GAZ:00067073</oboInOwl:id>
        <rdfs:label>Municipality of El Rama</rdfs:label>
    </owl:NamedIndividual>
    


    <!-- http://purl.obolibrary.org/obo/GAZ_00067074 -->

    <owl:NamedIndividual rdf:about="http://purl.obolibrary.org/obo/GAZ_00067074">
        <rdf:type rdf:resource="http://purl.obolibrary.org/obo/ENVO_00000856"/>
        <obo:RO_0001025 rdf:resource="http://purl.obolibrary.org/obo/GAZ_00047243"/>
        <obo:IAO_0000115>A municipality in Region Autonoma del Atlantico Sur, Nicaragua.</obo:IAO_0000115>
        <oboInOwl:hasOBONamespace>GAZ</oboInOwl:hasOBONamespace>
        <oboInOwl:id>GAZ:00067074</oboInOwl:id>
        <rdfs:label>Municipality of Desembocadura de la Cruz de Rio Grande</rdfs:label>
    </owl:NamedIndividual>
    


    <!-- http://purl.obolibrary.org/obo/GAZ_00067075 -->

    <owl:NamedIndividual rdf:about="http://purl.obolibrary.org/obo/GAZ_00067075">
        <rdf:type rdf:resource="http://purl.obolibrary.org/obo/ENVO_00000856"/>
        <obo:RO_0001025 rdf:resource="http://purl.obolibrary.org/obo/GAZ_00047243"/>
        <obo:IAO_0000115>A municipality in Region Autonoma del Atlantico Sur, Nicaragua.</obo:IAO_0000115>
        <oboInOwl:hasOBONamespace>GAZ</oboInOwl:hasOBONamespace>
        <oboInOwl:id>GAZ:00067075</oboInOwl:id>
        <rdfs:label>Municipality of El Ayote</rdfs:label>
    </owl:NamedIndividual>
    


    <!-- http://purl.obolibrary.org/obo/GAZ_00067076 -->

    <owl:NamedIndividual rdf:about="http://purl.obolibrary.org/obo/GAZ_00067076">
        <rdf:type rdf:resource="http://purl.obolibrary.org/obo/ENVO_00000856"/>
        <obo:RO_0001025 rdf:resource="http://purl.obolibrary.org/obo/GAZ_00047243"/>
        <obo:IAO_0000115>A municipality in Region Autonoma del Atlantico Sur, Nicaragua.</obo:IAO_0000115>
        <oboInOwl:hasOBONamespace>GAZ</oboInOwl:hasOBONamespace>
        <oboInOwl:id>GAZ:00067076</oboInOwl:id>
        <rdfs:label>Municipality of Nueva Guinea</rdfs:label>
    </owl:NamedIndividual>
    


    <!-- http://purl.obolibrary.org/obo/GAZ_00067077 -->

    <owl:NamedIndividual rdf:about="http://purl.obolibrary.org/obo/GAZ_00067077">
        <rdf:type rdf:resource="http://purl.obolibrary.org/obo/ENVO_00000856"/>
        <obo:RO_0001025 rdf:resource="http://purl.obolibrary.org/obo/GAZ_00047243"/>
        <obo:IAO_0000115>A municipality in Region Autonoma del Atlantico Sur, Nicaragua.</obo:IAO_0000115>
        <oboInOwl:hasOBONamespace>GAZ</oboInOwl:hasOBONamespace>
        <oboInOwl:id>GAZ:00067077</oboInOwl:id>
        <rdfs:label>Municipality of El Tortugero</rdfs:label>
    </owl:NamedIndividual>
    


    <!-- http://purl.obolibrary.org/obo/GAZ_00146307 -->

    <owl:NamedIndividual rdf:about="http://purl.obolibrary.org/obo/GAZ_00146307">
        <oboInOwl:hasOBONamespace>GAZ</oboInOwl:hasOBONamespace>
        <oboInOwl:id>GAZ:00146307</oboInOwl:id>
        <rdfs:label>Apoyo Lagoon</rdfs:label>
    </owl:NamedIndividual>
    


    <!-- http://purl.obolibrary.org/obo/GAZ_00146326 -->

    <owl:NamedIndividual rdf:about="http://purl.obolibrary.org/obo/GAZ_00146326">
        <obo:RO_0001025 rdf:resource="http://purl.obolibrary.org/obo/GAZ_00056200"/>
        <obo:RO_0001025 rdf:resource="http://purl.obolibrary.org/obo/GAZ_00267048"/>
        <obo:IAO_0000115>A protected area. Established 1991-10-31.</obo:IAO_0000115>
        <oboInOwl:hasOBONamespace>GAZ</oboInOwl:hasOBONamespace>
        <oboInOwl:id>GAZ:00146326</oboInOwl:id>
        <rdfs:label>Reserva Natural Laguna de Tiscapa</rdfs:label>
    </owl:NamedIndividual>
    


    <!-- http://purl.obolibrary.org/obo/GAZ_00146327 -->

    <owl:NamedIndividual rdf:about="http://purl.obolibrary.org/obo/GAZ_00146327">
        <obo:RO_0001025 rdf:resource="http://purl.obolibrary.org/obo/GAZ_00146326"/>
        <obo:IAO_0000115>A lagoon of volcanic origin that formed over 10,000 years ago.</obo:IAO_0000115>
        <oboInOwl:hasOBONamespace>GAZ</oboInOwl:hasOBONamespace>
        <oboInOwl:id>GAZ:00146327</oboInOwl:id>
        <rdfs:label>Laguna de Tiscapa</rdfs:label>
    </owl:NamedIndividual>
    


    <!-- http://purl.obolibrary.org/obo/GAZ_00264518 -->

    <owl:NamedIndividual rdf:about="http://purl.obolibrary.org/obo/GAZ_00264518">
        <obo:IAO_0000115>A river. A tributary of the San Juan River.</obo:IAO_0000115>
        <oboInOwl:hasOBONamespace>GAZ</oboInOwl:hasOBONamespace>
        <oboInOwl:id>GAZ:00264518</oboInOwl:id>
        <rdfs:label>Rio Sarapiqui</rdfs:label>
    </owl:NamedIndividual>
    


    <!-- http://purl.obolibrary.org/obo/GAZ_00264519 -->

    <owl:NamedIndividual rdf:about="http://purl.obolibrary.org/obo/GAZ_00264519">
        <obo:IAO_0000115>A river.</obo:IAO_0000115>
        <oboInOwl:hasOBONamespace>GAZ</oboInOwl:hasOBONamespace>
        <oboInOwl:id>GAZ:00264519</oboInOwl:id>
        <rdfs:label>Rio Toro</rdfs:label>
    </owl:NamedIndividual>
    


    <!-- http://purl.obolibrary.org/obo/GAZ_00264520 -->

    <owl:NamedIndividual rdf:about="http://purl.obolibrary.org/obo/GAZ_00264520">
        <obo:IAO_0000115>A river.</obo:IAO_0000115>
        <oboInOwl:hasOBONamespace>GAZ</oboInOwl:hasOBONamespace>
        <oboInOwl:id>GAZ:00264520</oboInOwl:id>
        <rdfs:label>Rio Sucio</rdfs:label>
    </owl:NamedIndividual>
    


    <!-- http://purl.obolibrary.org/obo/GAZ_00264521 -->

    <owl:NamedIndividual rdf:about="http://purl.obolibrary.org/obo/GAZ_00264521">
        <oboInOwl:hasOBONamespace>GAZ</oboInOwl:hasOBONamespace>
        <oboInOwl:id>GAZ:00264521</oboInOwl:id>
        <rdfs:label>Rio San Carlos</rdfs:label>
    </owl:NamedIndividual>
    


    <!-- http://purl.obolibrary.org/obo/GAZ_00264525 -->

    <owl:NamedIndividual rdf:about="http://purl.obolibrary.org/obo/GAZ_00264525">
        <obo:IAO_0000115>A river.</obo:IAO_0000115>
        <oboInOwl:hasOBONamespace>GAZ</oboInOwl:hasOBONamespace>
        <oboInOwl:id>GAZ:00264525</oboInOwl:id>
        <rdfs:label>Rio Celeste</rdfs:label>
    </owl:NamedIndividual>
    


    <!-- http://purl.obolibrary.org/obo/GAZ_00264526 -->

    <owl:NamedIndividual rdf:about="http://purl.obolibrary.org/obo/GAZ_00264526">
        <obo:IAO_0000115>A river.</obo:IAO_0000115>
        <oboInOwl:hasOBONamespace>GAZ</oboInOwl:hasOBONamespace>
        <oboInOwl:id>GAZ:00264526</oboInOwl:id>
        <rdfs:label>Rio Sabogal</rdfs:label>
    </owl:NamedIndividual>
    


    <!-- http://purl.obolibrary.org/obo/GAZ_00265029 -->

    <owl:NamedIndividual rdf:about="http://purl.obolibrary.org/obo/GAZ_00265029">
        <obo:RO_0001025 rdf:resource="http://purl.obolibrary.org/obo/GAZ_00047486"/>
        <obo:IAO_0000115>A bay.</obo:IAO_0000115>
        <oboInOwl:hasOBONamespace>GAZ</oboInOwl:hasOBONamespace>
        <oboInOwl:id>GAZ:00265029</oboInOwl:id>
        <rdfs:label>Bahia de la Union</rdfs:label>
    </owl:NamedIndividual>
    


    <!-- http://purl.obolibrary.org/obo/GAZ_00265353 -->

    <owl:NamedIndividual rdf:about="http://purl.obolibrary.org/obo/GAZ_00265353">
        <obo:RO_0001025 rdf:resource="http://purl.obolibrary.org/obo/GAZ_00047492"/>
        <obo:IAO_0000115>A Canton of the Municipality of Meanguera del Golfo.</obo:IAO_0000115>
        <oboInOwl:hasOBONamespace>GAZ</oboInOwl:hasOBONamespace>
        <oboInOwl:id>GAZ:00265353</oboInOwl:id>
        <rdfs:label>Isla de Conchaguita</rdfs:label>
    </owl:NamedIndividual>
    


    <!-- http://purl.obolibrary.org/obo/GAZ_00265672 -->

    <owl:NamedIndividual rdf:about="http://purl.obolibrary.org/obo/GAZ_00265672">
        <obo:IAO_0000115>A river.</obo:IAO_0000115>
        <oboInOwl:hasOBONamespace>GAZ</oboInOwl:hasOBONamespace>
        <oboInOwl:id>GAZ:00265672</oboInOwl:id>
        <rdfs:label>Rio El Sauce</rdfs:label>
    </owl:NamedIndividual>
    


    <!-- http://purl.obolibrary.org/obo/GAZ_00265673 -->

    <owl:NamedIndividual rdf:about="http://purl.obolibrary.org/obo/GAZ_00265673">
        <obo:IAO_0000115>A river.</obo:IAO_0000115>
        <oboInOwl:hasOBONamespace>GAZ</oboInOwl:hasOBONamespace>
        <oboInOwl:id>GAZ:00265673</oboInOwl:id>
        <rdfs:label>Rio Pasaquina</rdfs:label>
    </owl:NamedIndividual>
    


    <!-- http://purl.obolibrary.org/obo/GAZ_00265674 -->

    <owl:NamedIndividual rdf:about="http://purl.obolibrary.org/obo/GAZ_00265674">
        <obo:IAO_0000115>A river.</obo:IAO_0000115>
        <oboInOwl:hasOBONamespace>GAZ</oboInOwl:hasOBONamespace>
        <oboInOwl:id>GAZ:00265674</oboInOwl:id>
        <rdfs:label>Rio Sirama</rdfs:label>
    </owl:NamedIndividual>
    


    <!-- http://purl.obolibrary.org/obo/GAZ_00266759 -->

    <owl:NamedIndividual rdf:about="http://purl.obolibrary.org/obo/GAZ_00266759">
        <obo:IAO_0000115>A river.</obo:IAO_0000115>
        <oboInOwl:hasOBONamespace>GAZ</oboInOwl:hasOBONamespace>
        <oboInOwl:id>GAZ:00266759</oboInOwl:id>
        <rdfs:label>Rio Nacaome</rdfs:label>
    </owl:NamedIndividual>
    


    <!-- http://purl.obolibrary.org/obo/GAZ_00267030 -->

    <owl:NamedIndividual rdf:about="http://purl.obolibrary.org/obo/GAZ_00267030">
        <rdf:type rdf:resource="http://purl.obolibrary.org/obo/ENVO_00000856"/>
        <obo:RO_0001025 rdf:resource="http://purl.obolibrary.org/obo/GAZ_00047244"/>
        <obo:IAO_0000115>A municipality in the Region Autonoma del Atlantico Norte department of Nicaragua.</obo:IAO_0000115>
        <oboInOwl:hasOBONamespace>GAZ</oboInOwl:hasOBONamespace>
        <oboInOwl:id>GAZ:00267030</oboInOwl:id>
        <rdfs:label>Municipality of Krukira</rdfs:label>
    </owl:NamedIndividual>
    


    <!-- http://purl.obolibrary.org/obo/GAZ_00267031 -->

    <owl:NamedIndividual rdf:about="http://purl.obolibrary.org/obo/GAZ_00267031">
        <obo:RO_0001025 rdf:resource="http://purl.obolibrary.org/obo/GAZ_00002978"/>
        <obo:IAO_0000115>The central mountain range of Nicaragua.</obo:IAO_0000115>
        <oboInOwl:hasOBONamespace>GAZ</oboInOwl:hasOBONamespace>
        <oboInOwl:id>GAZ:00267031</oboInOwl:id>
        <rdfs:label>Cordillera Chontalena</rdfs:label>
    </owl:NamedIndividual>
    


    <!-- http://purl.obolibrary.org/obo/GAZ_00267032 -->

    <owl:NamedIndividual rdf:about="http://purl.obolibrary.org/obo/GAZ_00267032">
        <obo:RO_0001025 rdf:resource="http://purl.obolibrary.org/obo/GAZ_00066798"/>
        <obo:RO_0001025 rdf:resource="http://purl.obolibrary.org/obo/GAZ_00267031"/>
        <obo:IAO_0000115>A small mountain range in the central spine of Nicaragua, the Cordillera Chontalena, separating Lake Nicaragua from the Mosquito Coast.</obo:IAO_0000115>
        <oboInOwl:hasOBONamespace>GAZ</oboInOwl:hasOBONamespace>
        <oboInOwl:id>GAZ:00267032</oboInOwl:id>
        <rdfs:label>Serranias Amerrique</rdfs:label>
    </owl:NamedIndividual>
    


    <!-- http://purl.obolibrary.org/obo/GAZ_00267033 -->

    <owl:NamedIndividual rdf:about="http://purl.obolibrary.org/obo/GAZ_00267033">
        <obo:RO_0001025 rdf:resource="http://purl.obolibrary.org/obo/GAZ_00267031"/>
        <obo:IAO_0000115>A mountain range. The northern portion of the central mountain range in Nicaragua, which runs from north-west to south-east through the center of the country.</obo:IAO_0000115>
        <oboInOwl:hasOBONamespace>GAZ</oboInOwl:hasOBONamespace>
        <oboInOwl:id>GAZ:00267033</oboInOwl:id>
        <rdfs:label>Cordillera Isabelia</rdfs:label>
    </owl:NamedIndividual>
    


    <!-- http://purl.obolibrary.org/obo/GAZ_00267034 -->

    <owl:NamedIndividual rdf:about="http://purl.obolibrary.org/obo/GAZ_00267034">
        <obo:RO_0001025 rdf:resource="http://purl.obolibrary.org/obo/GAZ_00056211"/>
        <obo:IAO_0000115>A protected area. Established 1990.</obo:IAO_0000115>
        <oboInOwl:hasOBONamespace>GAZ</oboInOwl:hasOBONamespace>
        <oboInOwl:id>GAZ:00267034</oboInOwl:id>
        <rdfs:label>Miraflor Natural Reserve</rdfs:label>
    </owl:NamedIndividual>
    


    <!-- http://purl.obolibrary.org/obo/GAZ_00267035 -->

    <owl:NamedIndividual rdf:about="http://purl.obolibrary.org/obo/GAZ_00267035">
        <obo:RO_0001025 rdf:resource="http://purl.obolibrary.org/obo/GAZ_00066964"/>
        <obo:IAO_0000115>A populated place.</obo:IAO_0000115>
        <oboInOwl:hasOBONamespace>GAZ</oboInOwl:hasOBONamespace>
        <oboInOwl:id>GAZ:00267035</oboInOwl:id>
        <rdfs:label>Villa de San Antonio de Pavia de Esteli</rdfs:label>
    </owl:NamedIndividual>
    


    <!-- http://purl.obolibrary.org/obo/GAZ_00267036 -->

    <owl:NamedIndividual rdf:about="http://purl.obolibrary.org/obo/GAZ_00267036">
        <obo:RO_0001025 rdf:resource="http://purl.obolibrary.org/obo/GAZ_00066980"/>
        <obo:IAO_0000115>A protected area.</obo:IAO_0000115>
        <oboInOwl:hasOBONamespace>GAZ</oboInOwl:hasOBONamespace>
        <oboInOwl:id>GAZ:00267036</oboInOwl:id>
        <rdfs:label>Asososca Lagoon Natural Reserve</rdfs:label>
    </owl:NamedIndividual>
    


    <!-- http://purl.obolibrary.org/obo/GAZ_00267037 -->

    <owl:NamedIndividual rdf:about="http://purl.obolibrary.org/obo/GAZ_00267037">
        <rdf:type rdf:resource="http://purl.obolibrary.org/obo/ENVO_00000856"/>
        <obo:RO_0001025 rdf:resource="http://purl.obolibrary.org/obo/GAZ_00056193"/>
        <obo:IAO_0000115>A municipality in the Leon Department of Nicaragua.</obo:IAO_0000115>
        <oboInOwl:hasOBONamespace>GAZ</oboInOwl:hasOBONamespace>
        <oboInOwl:id>GAZ:00267037</oboInOwl:id>
        <rdfs:label>Municipality of Las Penitas</rdfs:label>
    </owl:NamedIndividual>
    


    <!-- http://purl.obolibrary.org/obo/GAZ_00267039 -->

    <owl:NamedIndividual rdf:about="http://purl.obolibrary.org/obo/GAZ_00267039">
        <obo:RO_0001025 rdf:resource="http://purl.obolibrary.org/obo/GAZ_00056190"/>
        <obo:IAO_0000115>A volcanic site.</obo:IAO_0000115>
        <oboInOwl:hasOBONamespace>GAZ</oboInOwl:hasOBONamespace>
        <oboInOwl:id>GAZ:00267039</oboInOwl:id>
        <rdfs:label>Los hervideros de San Jacinto</rdfs:label>
    </owl:NamedIndividual>
    


    <!-- http://purl.obolibrary.org/obo/GAZ_00267040 -->

    <owl:NamedIndividual rdf:about="http://purl.obolibrary.org/obo/GAZ_00267040">
        <obo:RO_0001025 rdf:resource="http://purl.obolibrary.org/obo/GAZ_00066990"/>
        <obo:IAO_0000115>A protected area that includes a canyon located in the Madriz Department of Nicaragua. Established 2005-11-29.</obo:IAO_0000115>
        <oboInOwl:hasOBONamespace>GAZ</oboInOwl:hasOBONamespace>
        <oboInOwl:id>GAZ:00267040</oboInOwl:id>
        <rdfs:label>Monumento Nacional Canon de Somoto</rdfs:label>
    </owl:NamedIndividual>
    


    <!-- http://purl.obolibrary.org/obo/GAZ_00267041 -->

    <owl:NamedIndividual rdf:about="http://purl.obolibrary.org/obo/GAZ_00267041">
        <obo:RO_0001025 rdf:resource="http://purl.obolibrary.org/obo/GAZ_00267040"/>
        <obo:IAO_0000115>A canyon.</obo:IAO_0000115>
        <oboInOwl:hasOBONamespace>GAZ</oboInOwl:hasOBONamespace>
        <oboInOwl:id>GAZ:00267041</oboInOwl:id>
        <rdfs:label>Canon de Somoto</rdfs:label>
    </owl:NamedIndividual>
    


    <!-- http://purl.obolibrary.org/obo/GAZ_00267042 -->

    <owl:NamedIndividual rdf:about="http://purl.obolibrary.org/obo/GAZ_00267042">
        <obo:RO_0001025 rdf:resource="http://purl.obolibrary.org/obo/GAZ_00267105"/>
        <obo:IAO_0000115>A lagoon.</obo:IAO_0000115>
        <oboInOwl:hasOBONamespace>GAZ</oboInOwl:hasOBONamespace>
        <oboInOwl:id>GAZ:00267042</oboInOwl:id>
        <rdfs:label>Laguna de Asososca</rdfs:label>
    </owl:NamedIndividual>
    


    <!-- http://purl.obolibrary.org/obo/GAZ_00267043 -->

    <owl:NamedIndividual rdf:about="http://purl.obolibrary.org/obo/GAZ_00267043">
        <obo:RO_0001025 rdf:resource="http://purl.obolibrary.org/obo/GAZ_00267104"/>
        <obo:IAO_0000115>A lagoon.</obo:IAO_0000115>
        <oboInOwl:hasOBONamespace>GAZ</oboInOwl:hasOBONamespace>
        <oboInOwl:id>GAZ:00267043</oboInOwl:id>
        <rdfs:label>Laguna de Nejapa</rdfs:label>
    </owl:NamedIndividual>
    


    <!-- http://purl.obolibrary.org/obo/GAZ_00267044 -->

    <owl:NamedIndividual rdf:about="http://purl.obolibrary.org/obo/GAZ_00267044">
        <obo:RO_0001025 rdf:resource="http://purl.obolibrary.org/obo/GAZ_00067004"/>
        <obo:IAO_0000115>A lagoon.</obo:IAO_0000115>
        <oboInOwl:hasOBONamespace>GAZ</oboInOwl:hasOBONamespace>
        <oboInOwl:id>GAZ:00267044</oboInOwl:id>
        <rdfs:label>Laguna de Acahualinca</rdfs:label>
    </owl:NamedIndividual>
    


    <!-- http://purl.obolibrary.org/obo/GAZ_00267045 -->

    <owl:NamedIndividual rdf:about="http://purl.obolibrary.org/obo/GAZ_00267045">
        <obo:RO_0001025 rdf:resource="http://purl.obolibrary.org/obo/GAZ_00056198"/>
        <obo:IAO_0000115>A lagoon.</obo:IAO_0000115>
        <oboInOwl:hasOBONamespace>GAZ</oboInOwl:hasOBONamespace>
        <oboInOwl:id>GAZ:00267045</oboInOwl:id>
        <rdfs:label>Laguna de Apoyeque</rdfs:label>
    </owl:NamedIndividual>
    


    <!-- http://purl.obolibrary.org/obo/GAZ_00267046 -->

    <owl:NamedIndividual rdf:about="http://purl.obolibrary.org/obo/GAZ_00267046">
        <obo:RO_0001025 rdf:resource="http://purl.obolibrary.org/obo/GAZ_00067013"/>
        <obo:IAO_0000115>A protected area. Established 1993.</obo:IAO_0000115>
        <oboInOwl:hasOBONamespace>GAZ</oboInOwl:hasOBONamespace>
        <oboInOwl:id>GAZ:00267046</oboInOwl:id>
        <rdfs:label>Reserva Natural El Chocoyero-El Brujo</rdfs:label>
    </owl:NamedIndividual>
    


    <!-- http://purl.obolibrary.org/obo/GAZ_00267047 -->

    <owl:NamedIndividual rdf:about="http://purl.obolibrary.org/obo/GAZ_00267047">
        <obo:RO_0001025 rdf:resource="http://purl.obolibrary.org/obo/GAZ_00067004"/>
        <obo:IAO_0000115>A populated place. The capital city of Nicaragua.</obo:IAO_0000115>
        <oboInOwl:hasOBONamespace>GAZ</oboInOwl:hasOBONamespace>
        <oboInOwl:id>GAZ:00267047</oboInOwl:id>
        <rdfs:label>Managua</rdfs:label>
    </owl:NamedIndividual>
    


    <!-- http://purl.obolibrary.org/obo/GAZ_00267048 -->

    <owl:NamedIndividual rdf:about="http://purl.obolibrary.org/obo/GAZ_00267048">
        <rdf:type rdf:resource="http://purl.obolibrary.org/obo/ENVO_00000004"/>
        <obo:RO_0001025 rdf:resource="http://purl.obolibrary.org/obo/GAZ_00267047"/>
        <obo:IAO_0000115>A district of Managua.</obo:IAO_0000115>
        <oboInOwl:hasOBONamespace>GAZ</oboInOwl:hasOBONamespace>
        <oboInOwl:id>GAZ:00267048</oboInOwl:id>
        <rdfs:label>Distrito I</rdfs:label>
    </owl:NamedIndividual>
    


    <!-- http://purl.obolibrary.org/obo/GAZ_00267049 -->

    <owl:NamedIndividual rdf:about="http://purl.obolibrary.org/obo/GAZ_00267049">
        <rdf:type rdf:resource="http://purl.obolibrary.org/obo/ENVO_00000004"/>
        <obo:RO_0001025 rdf:resource="http://purl.obolibrary.org/obo/GAZ_00267047"/>
        <obo:IAO_0000115>A district of Managua.</obo:IAO_0000115>
        <oboInOwl:hasOBONamespace>GAZ</oboInOwl:hasOBONamespace>
        <oboInOwl:id>GAZ:00267049</oboInOwl:id>
        <rdfs:label>Distrito II</rdfs:label>
    </owl:NamedIndividual>
    


    <!-- http://purl.obolibrary.org/obo/GAZ_00267050 -->

    <owl:NamedIndividual rdf:about="http://purl.obolibrary.org/obo/GAZ_00267050">
        <rdf:type rdf:resource="http://purl.obolibrary.org/obo/ENVO_00000004"/>
        <obo:RO_0001025 rdf:resource="http://purl.obolibrary.org/obo/GAZ_00267047"/>
        <obo:IAO_0000115>A district of Managua.</obo:IAO_0000115>
        <oboInOwl:hasOBONamespace>GAZ</oboInOwl:hasOBONamespace>
        <oboInOwl:id>GAZ:00267050</oboInOwl:id>
        <rdfs:label>Distrito III</rdfs:label>
    </owl:NamedIndividual>
    


    <!-- http://purl.obolibrary.org/obo/GAZ_00267051 -->

    <owl:NamedIndividual rdf:about="http://purl.obolibrary.org/obo/GAZ_00267051">
        <rdf:type rdf:resource="http://purl.obolibrary.org/obo/ENVO_00000004"/>
        <obo:RO_0001025 rdf:resource="http://purl.obolibrary.org/obo/GAZ_00267047"/>
        <obo:IAO_0000115>A district of Managua.</obo:IAO_0000115>
        <oboInOwl:hasOBONamespace>GAZ</oboInOwl:hasOBONamespace>
        <oboInOwl:id>GAZ:00267051</oboInOwl:id>
        <rdfs:label>Distrito IV</rdfs:label>
    </owl:NamedIndividual>
    


    <!-- http://purl.obolibrary.org/obo/GAZ_00267052 -->

    <owl:NamedIndividual rdf:about="http://purl.obolibrary.org/obo/GAZ_00267052">
        <rdf:type rdf:resource="http://purl.obolibrary.org/obo/ENVO_00000004"/>
        <obo:RO_0001025 rdf:resource="http://purl.obolibrary.org/obo/GAZ_00267047"/>
        <obo:IAO_0000115>A district of Managua.</obo:IAO_0000115>
        <oboInOwl:hasOBONamespace>GAZ</oboInOwl:hasOBONamespace>
        <oboInOwl:id>GAZ:00267052</oboInOwl:id>
        <rdfs:label>Distrito V</rdfs:label>
    </owl:NamedIndividual>
    


    <!-- http://purl.obolibrary.org/obo/GAZ_00267053 -->

    <owl:NamedIndividual rdf:about="http://purl.obolibrary.org/obo/GAZ_00267053">
        <rdf:type rdf:resource="http://purl.obolibrary.org/obo/ENVO_00000004"/>
        <obo:RO_0001025 rdf:resource="http://purl.obolibrary.org/obo/GAZ_00267047"/>
        <obo:IAO_0000115>A district of Managua.</obo:IAO_0000115>
        <oboInOwl:hasOBONamespace>GAZ</oboInOwl:hasOBONamespace>
        <oboInOwl:id>GAZ:00267053</oboInOwl:id>
        <rdfs:label>Distrito VI</rdfs:label>
    </owl:NamedIndividual>
    


    <!-- http://purl.obolibrary.org/obo/GAZ_00267054 -->

    <owl:NamedIndividual rdf:about="http://purl.obolibrary.org/obo/GAZ_00267054">
        <rdf:type rdf:resource="http://purl.obolibrary.org/obo/ENVO_00000004"/>
        <obo:RO_0001025 rdf:resource="http://purl.obolibrary.org/obo/GAZ_00267047"/>
        <obo:IAO_0000115>A district of Managua.</obo:IAO_0000115>
        <oboInOwl:hasOBONamespace>GAZ</oboInOwl:hasOBONamespace>
        <oboInOwl:id>GAZ:00267054</oboInOwl:id>
        <rdfs:label>Distrito VII</rdfs:label>
    </owl:NamedIndividual>
    


    <!-- http://purl.obolibrary.org/obo/GAZ_00267055 -->

    <owl:NamedIndividual rdf:about="http://purl.obolibrary.org/obo/GAZ_00267055">
        <obo:RO_0001025 rdf:resource="http://purl.obolibrary.org/obo/GAZ_00067008"/>
        <obo:IAO_0000115>A protected area. Established 1979-05-23.</obo:IAO_0000115>
        <oboInOwl:hasOBONamespace>GAZ</oboInOwl:hasOBONamespace>
        <oboInOwl:id>GAZ:00267055</oboInOwl:id>
        <rdfs:label>Parque Nacional Volcan Masaya</rdfs:label>
    </owl:NamedIndividual>
    


    <!-- http://purl.obolibrary.org/obo/GAZ_00267056 -->

    <owl:NamedIndividual rdf:about="http://purl.obolibrary.org/obo/GAZ_00267056">
        <obo:RO_0001025 rdf:resource="http://purl.obolibrary.org/obo/GAZ_00047261"/>
        <obo:IAO_0000115>A protected area.</obo:IAO_0000115>
        <oboInOwl:hasOBONamespace>GAZ</oboInOwl:hasOBONamespace>
        <oboInOwl:id>GAZ:00267056</oboInOwl:id>
        <rdfs:label>Reserva de la Biosfera de Rio San Juan</rdfs:label>
    </owl:NamedIndividual>
    


    <!-- http://purl.obolibrary.org/obo/GAZ_00267057 -->

    <owl:NamedIndividual rdf:about="http://purl.obolibrary.org/obo/GAZ_00267057">
        <obo:RO_0001025 rdf:resource="http://purl.obolibrary.org/obo/GAZ_00067056"/>
        <obo:RO_0001025 rdf:resource="http://purl.obolibrary.org/obo/GAZ_00267056"/>
        <obo:IAO_0000115>A protected area. A Ramsar Site.</obo:IAO_0000115>
        <oboInOwl:hasOBONamespace>GAZ</oboInOwl:hasOBONamespace>
        <oboInOwl:id>GAZ:00267057</oboInOwl:id>
        <rdfs:label>Refugio de vida salvaje Los Guatuzos</rdfs:label>
    </owl:NamedIndividual>
    


    <!-- http://purl.obolibrary.org/obo/GAZ_00267060 -->

    <owl:NamedIndividual rdf:about="http://purl.obolibrary.org/obo/GAZ_00267060">
        <rdf:type rdf:resource="http://purl.obolibrary.org/obo/ENVO_00000098"/>
        <obo:RO_0001025 rdf:resource="http://purl.obolibrary.org/obo/GAZ_00047254"/>
        <obo:IAO_0000115>A cay.</obo:IAO_0000115>
        <oboInOwl:hasOBONamespace>GAZ</oboInOwl:hasOBONamespace>
        <oboInOwl:id>GAZ:00267060</oboInOwl:id>
        <rdfs:label>Cayo Crawl</rdfs:label>
    </owl:NamedIndividual>
    


    <!-- http://purl.obolibrary.org/obo/GAZ_00267061 -->

    <owl:NamedIndividual rdf:about="http://purl.obolibrary.org/obo/GAZ_00267061">
        <rdf:type rdf:resource="http://purl.obolibrary.org/obo/ENVO_00000098"/>
        <obo:RO_0001025 rdf:resource="http://purl.obolibrary.org/obo/GAZ_00047254"/>
        <obo:IAO_0000115>A cay.</obo:IAO_0000115>
        <oboInOwl:hasOBONamespace>GAZ</oboInOwl:hasOBONamespace>
        <oboInOwl:id>GAZ:00267061</oboInOwl:id>
        <rdfs:label>Cayo Baboon</rdfs:label>
    </owl:NamedIndividual>
    


    <!-- http://purl.obolibrary.org/obo/GAZ_00267062 -->

    <owl:NamedIndividual rdf:about="http://purl.obolibrary.org/obo/GAZ_00267062">
        <rdf:type rdf:resource="http://purl.obolibrary.org/obo/ENVO_00000098"/>
        <obo:RO_0001025 rdf:resource="http://purl.obolibrary.org/obo/GAZ_00047254"/>
        <obo:IAO_0000115>A cay.</obo:IAO_0000115>
        <oboInOwl:hasOBONamespace>GAZ</oboInOwl:hasOBONamespace>
        <oboInOwl:id>GAZ:00267062</oboInOwl:id>
        <rdfs:label>Cayo Grape</rdfs:label>
    </owl:NamedIndividual>
    


    <!-- http://purl.obolibrary.org/obo/GAZ_00267063 -->

    <owl:NamedIndividual rdf:about="http://purl.obolibrary.org/obo/GAZ_00267063">
        <rdf:type rdf:resource="http://purl.obolibrary.org/obo/ENVO_00000098"/>
        <obo:RO_0001025 rdf:resource="http://purl.obolibrary.org/obo/GAZ_00047254"/>
        <obo:IAO_0000115>A cay.</obo:IAO_0000115>
        <oboInOwl:hasOBONamespace>GAZ</oboInOwl:hasOBONamespace>
        <oboInOwl:id>GAZ:00267063</oboInOwl:id>
        <rdfs:label>Cayo Water</rdfs:label>
    </owl:NamedIndividual>
    


    <!-- http://purl.obolibrary.org/obo/GAZ_00267064 -->

    <owl:NamedIndividual rdf:about="http://purl.obolibrary.org/obo/GAZ_00267064">
        <rdf:type rdf:resource="http://purl.obolibrary.org/obo/ENVO_00000098"/>
        <obo:RO_0001025 rdf:resource="http://purl.obolibrary.org/obo/GAZ_00047254"/>
        <obo:IAO_0000115>A cay.</obo:IAO_0000115>
        <oboInOwl:hasOBONamespace>GAZ</oboInOwl:hasOBONamespace>
        <oboInOwl:id>GAZ:00267064</oboInOwl:id>
        <rdfs:label>Cayo Vincent</rdfs:label>
    </owl:NamedIndividual>
    


    <!-- http://purl.obolibrary.org/obo/GAZ_00267065 -->

    <owl:NamedIndividual rdf:about="http://purl.obolibrary.org/obo/GAZ_00267065">
        <rdf:type rdf:resource="http://purl.obolibrary.org/obo/ENVO_00000098"/>
        <obo:RO_0001025 rdf:resource="http://purl.obolibrary.org/obo/GAZ_00047254"/>
        <obo:IAO_0000115>A cay.</obo:IAO_0000115>
        <oboInOwl:hasOBONamespace>GAZ</oboInOwl:hasOBONamespace>
        <oboInOwl:id>GAZ:00267065</oboInOwl:id>
        <rdfs:label>Cayo Wild Cane</rdfs:label>
    </owl:NamedIndividual>
    


    <!-- http://purl.obolibrary.org/obo/GAZ_00267066 -->

    <owl:NamedIndividual rdf:about="http://purl.obolibrary.org/obo/GAZ_00267066">
        <rdf:type rdf:resource="http://purl.obolibrary.org/obo/ENVO_00000098"/>
        <obo:RO_0001025 rdf:resource="http://purl.obolibrary.org/obo/GAZ_00047254"/>
        <obo:IAO_0000115>A cay.</obo:IAO_0000115>
        <oboInOwl:hasOBONamespace>GAZ</oboInOwl:hasOBONamespace>
        <oboInOwl:id>GAZ:00267066</oboInOwl:id>
        <rdfs:label>Cayo Lime</rdfs:label>
    </owl:NamedIndividual>
    


    <!-- http://purl.obolibrary.org/obo/GAZ_00267067 -->

    <owl:NamedIndividual rdf:about="http://purl.obolibrary.org/obo/GAZ_00267067">
        <rdf:type rdf:resource="http://purl.obolibrary.org/obo/ENVO_00000098"/>
        <obo:RO_0001025 rdf:resource="http://purl.obolibrary.org/obo/GAZ_00047254"/>
        <obo:IAO_0000115>A cay.</obo:IAO_0000115>
        <oboInOwl:hasOBONamespace>GAZ</oboInOwl:hasOBONamespace>
        <oboInOwl:id>GAZ:00267067</oboInOwl:id>
        <rdfs:label>Cayo Babumki</rdfs:label>
    </owl:NamedIndividual>
    


    <!-- http://purl.obolibrary.org/obo/GAZ_00267068 -->

    <owl:NamedIndividual rdf:about="http://purl.obolibrary.org/obo/GAZ_00267068">
        <rdf:type rdf:resource="http://purl.obolibrary.org/obo/ENVO_00000098"/>
        <obo:RO_0001025 rdf:resource="http://purl.obolibrary.org/obo/GAZ_00047254"/>
        <obo:IAO_0000115>A cay.</obo:IAO_0000115>
        <oboInOwl:hasOBONamespace>GAZ</oboInOwl:hasOBONamespace>
        <oboInOwl:id>GAZ:00267068</oboInOwl:id>
        <rdfs:label>Cayo Crawlicay</rdfs:label>
    </owl:NamedIndividual>
    


    <!-- http://purl.obolibrary.org/obo/GAZ_00267069 -->

    <owl:NamedIndividual rdf:about="http://purl.obolibrary.org/obo/GAZ_00267069">
        <rdf:type rdf:resource="http://purl.obolibrary.org/obo/ENVO_00000098"/>
        <obo:RO_0001025 rdf:resource="http://purl.obolibrary.org/obo/GAZ_00047254"/>
        <obo:IAO_0000115>A cay.</obo:IAO_0000115>
        <oboInOwl:hasOBONamespace>GAZ</oboInOwl:hasOBONamespace>
        <oboInOwl:id>GAZ:00267069</oboInOwl:id>
        <rdfs:label>Cayo Grapecay</rdfs:label>
    </owl:NamedIndividual>
    


    <!-- http://purl.obolibrary.org/obo/GAZ_00267070 -->

    <owl:NamedIndividual rdf:about="http://purl.obolibrary.org/obo/GAZ_00267070">
        <rdf:type rdf:resource="http://purl.obolibrary.org/obo/ENVO_00000098"/>
        <obo:RO_0001025 rdf:resource="http://purl.obolibrary.org/obo/GAZ_00047254"/>
        <obo:IAO_0000115>A cay.</obo:IAO_0000115>
        <oboInOwl:hasOBONamespace>GAZ</oboInOwl:hasOBONamespace>
        <oboInOwl:id>GAZ:00267070</oboInOwl:id>
        <rdfs:label>Cayo Sanfly 1</rdfs:label>
    </owl:NamedIndividual>
    


    <!-- http://purl.obolibrary.org/obo/GAZ_00267071 -->

    <owl:NamedIndividual rdf:about="http://purl.obolibrary.org/obo/GAZ_00267071">
        <rdf:type rdf:resource="http://purl.obolibrary.org/obo/ENVO_00000098"/>
        <obo:RO_0001025 rdf:resource="http://purl.obolibrary.org/obo/GAZ_00047254"/>
        <obo:IAO_0000115>A cay.</obo:IAO_0000115>
        <oboInOwl:hasOBONamespace>GAZ</oboInOwl:hasOBONamespace>
        <oboInOwl:id>GAZ:00267071</oboInOwl:id>
        <rdfs:label>Cayo Sanfly 2</rdfs:label>
    </owl:NamedIndividual>
    


    <!-- http://purl.obolibrary.org/obo/GAZ_00267072 -->

    <owl:NamedIndividual rdf:about="http://purl.obolibrary.org/obo/GAZ_00267072">
        <rdf:type rdf:resource="http://purl.obolibrary.org/obo/ENVO_00000098"/>
        <obo:RO_0001025 rdf:resource="http://purl.obolibrary.org/obo/GAZ_00047254"/>
        <obo:IAO_0000115>A cay.</obo:IAO_0000115>
        <oboInOwl:hasOBONamespace>GAZ</oboInOwl:hasOBONamespace>
        <oboInOwl:id>GAZ:00267072</oboInOwl:id>
        <rdfs:label>Cayo Coco</rdfs:label>
    </owl:NamedIndividual>
    


    <!-- http://purl.obolibrary.org/obo/GAZ_00267073 -->

    <owl:NamedIndividual rdf:about="http://purl.obolibrary.org/obo/GAZ_00267073">
        <rdf:type rdf:resource="http://purl.obolibrary.org/obo/ENVO_00000098"/>
        <obo:RO_0001025 rdf:resource="http://purl.obolibrary.org/obo/GAZ_00047254"/>
        <obo:IAO_0000115>A cay.</obo:IAO_0000115>
        <oboInOwl:hasOBONamespace>GAZ</oboInOwl:hasOBONamespace>
        <oboInOwl:id>GAZ:00267073</oboInOwl:id>
        <rdfs:label>Cayo Cohiba</rdfs:label>
    </owl:NamedIndividual>
    


    <!-- http://purl.obolibrary.org/obo/GAZ_00267074 -->

    <owl:NamedIndividual rdf:about="http://purl.obolibrary.org/obo/GAZ_00267074">
        <rdf:type rdf:resource="http://purl.obolibrary.org/obo/ENVO_00000098"/>
        <obo:RO_0001025 rdf:resource="http://purl.obolibrary.org/obo/GAZ_00047254"/>
        <obo:IAO_0000115>A cay.</obo:IAO_0000115>
        <oboInOwl:hasOBONamespace>GAZ</oboInOwl:hasOBONamespace>
        <oboInOwl:id>GAZ:00267074</oboInOwl:id>
        <rdfs:label>Cayo Vincent Vincent</rdfs:label>
    </owl:NamedIndividual>
    


    <!-- http://purl.obolibrary.org/obo/GAZ_00267075 -->

    <owl:NamedIndividual rdf:about="http://purl.obolibrary.org/obo/GAZ_00267075">
        <rdf:type rdf:resource="http://purl.obolibrary.org/obo/ENVO_00000098"/>
        <obo:RO_0001025 rdf:resource="http://purl.obolibrary.org/obo/GAZ_00047254"/>
        <obo:IAO_0000115>A cay.</obo:IAO_0000115>
        <oboInOwl:hasOBONamespace>GAZ</oboInOwl:hasOBONamespace>
        <oboInOwl:id>GAZ:00267075</oboInOwl:id>
        <rdfs:label>Cayo Lime Janike</rdfs:label>
    </owl:NamedIndividual>
    


    <!-- http://purl.obolibrary.org/obo/GAZ_00267077 -->

    <owl:NamedIndividual rdf:about="http://purl.obolibrary.org/obo/GAZ_00267077">
        <obo:IAO_0000115>A lake.</obo:IAO_0000115>
        <oboInOwl:hasOBONamespace>GAZ</oboInOwl:hasOBONamespace>
        <oboInOwl:id>GAZ:00267077</oboInOwl:id>
        <rdfs:label>Laguna Sunie</rdfs:label>
    </owl:NamedIndividual>
    


    <!-- http://purl.obolibrary.org/obo/GAZ_00267078 -->

    <owl:NamedIndividual rdf:about="http://purl.obolibrary.org/obo/GAZ_00267078">
        <obo:RO_0001025 rdf:resource="http://purl.obolibrary.org/obo/GAZ_00066943"/>
        <obo:IAO_0000115>A protected area. Established 1983-09-09.</obo:IAO_0000115>
        <oboInOwl:hasOBONamespace>GAZ</oboInOwl:hasOBONamespace>
        <oboInOwl:id>GAZ:00267078</oboInOwl:id>
        <rdfs:label>Reserva Natural Estero Padre Ramos</rdfs:label>
    </owl:NamedIndividual>
    


    <!-- http://purl.obolibrary.org/obo/GAZ_00267080 -->

    <owl:NamedIndividual rdf:about="http://purl.obolibrary.org/obo/GAZ_00267080">
        <obo:RO_0001025 rdf:resource="http://purl.obolibrary.org/obo/GAZ_00066943"/>
        <obo:IAO_0000115>A protected area. Established 2006-11-24.</obo:IAO_0000115>
        <oboInOwl:hasOBONamespace>GAZ</oboInOwl:hasOBONamespace>
        <oboInOwl:id>GAZ:00267080</oboInOwl:id>
        <rdfs:label>Reserva Natural Volcan Cosiguina</rdfs:label>
    </owl:NamedIndividual>
    


    <!-- http://purl.obolibrary.org/obo/GAZ_00267084 -->

    <owl:NamedIndividual rdf:about="http://purl.obolibrary.org/obo/GAZ_00267084">
        <obo:RO_0001025 rdf:resource="http://purl.obolibrary.org/obo/GAZ_00066970"/>
        <obo:IAO_0000115>A protected area. Established 1981.</obo:IAO_0000115>
        <oboInOwl:hasOBONamespace>GAZ</oboInOwl:hasOBONamespace>
        <oboInOwl:id>GAZ:00267084</oboInOwl:id>
        <rdfs:label>Parque Nacional Archipielago Zapatera</rdfs:label>
    </owl:NamedIndividual>
    


    <!-- http://purl.obolibrary.org/obo/GAZ_00267086 -->

    <owl:NamedIndividual rdf:about="http://purl.obolibrary.org/obo/GAZ_00267086">
        <obo:RO_0001025 rdf:resource="http://purl.obolibrary.org/obo/GAZ_00067042"/>
        <obo:IAO_0000115>A protected area. Established 2007-06-15.</obo:IAO_0000115>
        <oboInOwl:hasOBONamespace>GAZ</oboInOwl:hasOBONamespace>
        <oboInOwl:id>GAZ:00267086</oboInOwl:id>
        <rdfs:label>Refugio de Vida Silvestre La Flor</rdfs:label>
    </owl:NamedIndividual>
    


    <!-- http://purl.obolibrary.org/obo/GAZ_00267089 -->

    <owl:NamedIndividual rdf:about="http://purl.obolibrary.org/obo/GAZ_00267089">
        <obo:RO_0001025 rdf:resource="http://purl.obolibrary.org/obo/GAZ_00067029"/>
        <obo:IAO_0000115>A protected area.</obo:IAO_0000115>
        <oboInOwl:hasOBONamespace>GAZ</oboInOwl:hasOBONamespace>
        <oboInOwl:id>GAZ:00267089</oboInOwl:id>
        <rdfs:label>Reserva Natural Cerro Arenal</rdfs:label>
    </owl:NamedIndividual>
    


    <!-- http://purl.obolibrary.org/obo/GAZ_00267090 -->

    <owl:NamedIndividual rdf:about="http://purl.obolibrary.org/obo/GAZ_00267090">
        <obo:RO_0001025 rdf:resource="http://purl.obolibrary.org/obo/GAZ_00067017"/>
        <obo:IAO_0000115>A protected area.</obo:IAO_0000115>
        <oboInOwl:hasOBONamespace>GAZ</oboInOwl:hasOBONamespace>
        <oboInOwl:id>GAZ:00267090</oboInOwl:id>
        <rdfs:label>Reserva Natural Cerro Musun</rdfs:label>
    </owl:NamedIndividual>
    


    <!-- http://purl.obolibrary.org/obo/GAZ_00267091 -->

    <owl:NamedIndividual rdf:about="http://purl.obolibrary.org/obo/GAZ_00267091">
        <obo:RO_0001025 rdf:resource="http://purl.obolibrary.org/obo/GAZ_00067029"/>
        <obo:IAO_0000115>A protected area.</obo:IAO_0000115>
        <oboInOwl:hasOBONamespace>GAZ</oboInOwl:hasOBONamespace>
        <oboInOwl:id>GAZ:00267091</oboInOwl:id>
        <rdfs:label>Reserva Natural Cerro Apante</rdfs:label>
    </owl:NamedIndividual>
    


    <!-- http://purl.obolibrary.org/obo/GAZ_00267093 -->

    <owl:NamedIndividual rdf:about="http://purl.obolibrary.org/obo/GAZ_00267093">
        <obo:RO_0001025 rdf:resource="http://purl.obolibrary.org/obo/GAZ_00056197"/>
        <obo:RO_0001025 rdf:resource="http://purl.obolibrary.org/obo/GAZ_00067007"/>
        <obo:IAO_0000115>A protected area.</obo:IAO_0000115>
        <oboInOwl:hasOBONamespace>GAZ</oboInOwl:hasOBONamespace>
        <oboInOwl:id>GAZ:00267093</oboInOwl:id>
        <rdfs:label>Reserva Natural Peninsula de Chiltepe</rdfs:label>
    </owl:NamedIndividual>
    


    <!-- http://purl.obolibrary.org/obo/GAZ_00267096 -->

    <owl:NamedIndividual rdf:about="http://purl.obolibrary.org/obo/GAZ_00267096">
        <obo:RO_0001025 rdf:resource="http://purl.obolibrary.org/obo/GAZ_00067018"/>
        <obo:IAO_0000115>A protected area.</obo:IAO_0000115>
        <oboInOwl:hasOBONamespace>GAZ</oboInOwl:hasOBONamespace>
        <oboInOwl:id>GAZ:00267096</oboInOwl:id>
        <rdfs:label>Reserva de Recursos Geneticos Yucul</rdfs:label>
    </owl:NamedIndividual>
    


    <!-- http://purl.obolibrary.org/obo/GAZ_00267097 -->

    <owl:NamedIndividual rdf:about="http://purl.obolibrary.org/obo/GAZ_00267097">
        <obo:RO_0001025 rdf:resource="http://purl.obolibrary.org/obo/GAZ_00067056"/>
        <obo:IAO_0000115>A protected area.</obo:IAO_0000115>
        <oboInOwl:hasOBONamespace>GAZ</oboInOwl:hasOBONamespace>
        <oboInOwl:id>GAZ:00267097</oboInOwl:id>
        <rdfs:label>Monumento Nacional Archipielago de Solentiname</rdfs:label>
    </owl:NamedIndividual>
    


    <!-- http://purl.obolibrary.org/obo/GAZ_00267101 -->

    <owl:NamedIndividual rdf:about="http://purl.obolibrary.org/obo/GAZ_00267101">
        <obo:RO_0001025 rdf:resource="http://purl.obolibrary.org/obo/GAZ_00066947"/>
        <obo:IAO_0000115>A protected area.</obo:IAO_0000115>
        <oboInOwl:hasOBONamespace>GAZ</oboInOwl:hasOBONamespace>
        <oboInOwl:id>GAZ:00267101</oboInOwl:id>
        <rdfs:label>Monumento Nacional In Memoriam a las Victimas del huracan Mitch</rdfs:label>
    </owl:NamedIndividual>
    


    <!-- http://purl.obolibrary.org/obo/GAZ_00267102 -->

    <owl:NamedIndividual rdf:about="http://purl.obolibrary.org/obo/GAZ_00267102">
        <obo:RO_0001025 rdf:resource="http://purl.obolibrary.org/obo/GAZ_00066980"/>
        <obo:IAO_0000115>A protected area.</obo:IAO_0000115>
        <oboInOwl:hasOBONamespace>GAZ</oboInOwl:hasOBONamespace>
        <oboInOwl:id>GAZ:00267102</oboInOwl:id>
        <rdfs:label>Reserva Natural Complejo Volcanico Momotombo-Momotombito</rdfs:label>
    </owl:NamedIndividual>
    


    <!-- http://purl.obolibrary.org/obo/GAZ_00267104 -->

    <owl:NamedIndividual rdf:about="http://purl.obolibrary.org/obo/GAZ_00267104">
        <obo:RO_0001025 rdf:resource="http://purl.obolibrary.org/obo/GAZ_00267050"/>
        <obo:IAO_0000115>A protected area.</obo:IAO_0000115>
        <oboInOwl:hasOBONamespace>GAZ</oboInOwl:hasOBONamespace>
        <oboInOwl:id>GAZ:00267104</oboInOwl:id>
        <rdfs:label>Reserva Natural Laguna de Nejapa</rdfs:label>
    </owl:NamedIndividual>
    


    <!-- http://purl.obolibrary.org/obo/GAZ_00267105 -->

    <owl:NamedIndividual rdf:about="http://purl.obolibrary.org/obo/GAZ_00267105">
        <obo:RO_0001025 rdf:resource="http://purl.obolibrary.org/obo/GAZ_00267049"/>
        <obo:IAO_0000115>A protected area.</obo:IAO_0000115>
        <oboInOwl:hasOBONamespace>GAZ</oboInOwl:hasOBONamespace>
        <oboInOwl:id>GAZ:00267105</oboInOwl:id>
        <rdfs:label>Reserva Natural Laguna de Asososca</rdfs:label>
    </owl:NamedIndividual>
    


    <!-- http://purl.obolibrary.org/obo/GAZ_00267106 -->

    <owl:NamedIndividual rdf:about="http://purl.obolibrary.org/obo/GAZ_00267106">
        <obo:RO_0001025 rdf:resource="http://purl.obolibrary.org/obo/GAZ_00067051"/>
        <obo:IAO_0000115>A protected area.</obo:IAO_0000115>
        <oboInOwl:hasOBONamespace>GAZ</oboInOwl:hasOBONamespace>
        <oboInOwl:id>GAZ:00267106</oboInOwl:id>
        <rdfs:label>Reserva Natural Volcan Maderas</rdfs:label>
    </owl:NamedIndividual>
    


    <!-- http://purl.obolibrary.org/obo/GAZ_00267112 -->

    <owl:NamedIndividual rdf:about="http://purl.obolibrary.org/obo/GAZ_00267112">
        <obo:RO_0001025 rdf:resource="http://purl.obolibrary.org/obo/GAZ_00067026"/>
        <obo:IAO_0000115>A protected area.</obo:IAO_0000115>
        <oboInOwl:hasOBONamespace>GAZ</oboInOwl:hasOBONamespace>
        <oboInOwl:id>GAZ:00267112</oboInOwl:id>
        <rdfs:label>Reserva Natural Cerro Pancasan</rdfs:label>
    </owl:NamedIndividual>
    


    <!-- http://purl.obolibrary.org/obo/GAZ_00267113 -->

    <owl:NamedIndividual rdf:about="http://purl.obolibrary.org/obo/GAZ_00267113">
        <obo:RO_0001025 rdf:resource="http://purl.obolibrary.org/obo/GAZ_00056193"/>
        <obo:IAO_0000115>A protected area.</obo:IAO_0000115>
        <oboInOwl:hasOBONamespace>GAZ</oboInOwl:hasOBONamespace>
        <oboInOwl:id>GAZ:00267113</oboInOwl:id>
        <rdfs:label>Reserva Natural Complejo Volcanico Telica-Rota</rdfs:label>
    </owl:NamedIndividual>
    


    <!-- http://purl.obolibrary.org/obo/GAZ_00267114 -->

    <owl:NamedIndividual rdf:about="http://purl.obolibrary.org/obo/GAZ_00267114">
        <obo:RO_0001025 rdf:resource="http://purl.obolibrary.org/obo/GAZ_00056204"/>
        <obo:IAO_0000115>A protected area.</obo:IAO_0000115>
        <oboInOwl:hasOBONamespace>GAZ</oboInOwl:hasOBONamespace>
        <oboInOwl:id>GAZ:00267114</oboInOwl:id>
        <rdfs:label>Reserva Natural Lagunetas de Mecatepe</rdfs:label>
    </owl:NamedIndividual>
    


    <!-- http://purl.obolibrary.org/obo/GAZ_00267115 -->

    <owl:NamedIndividual rdf:about="http://purl.obolibrary.org/obo/GAZ_00267115">
        <obo:RO_0001025 rdf:resource="http://purl.obolibrary.org/obo/GAZ_00056204"/>
        <obo:IAO_0000115>A protected area.</obo:IAO_0000115>
        <oboInOwl:hasOBONamespace>GAZ</oboInOwl:hasOBONamespace>
        <oboInOwl:id>GAZ:00267115</oboInOwl:id>
        <rdfs:label>Reserva Natural Rio Manares</rdfs:label>
    </owl:NamedIndividual>
    


    <!-- http://purl.obolibrary.org/obo/GAZ_00267116 -->

    <owl:NamedIndividual rdf:about="http://purl.obolibrary.org/obo/GAZ_00267116">
        <obo:RO_0001025 rdf:resource="http://purl.obolibrary.org/obo/GAZ_00056208"/>
        <obo:IAO_0000115>A protected area.</obo:IAO_0000115>
        <oboInOwl:hasOBONamespace>GAZ</oboInOwl:hasOBONamespace>
        <oboInOwl:id>GAZ:00267116</oboInOwl:id>
        <rdfs:label>Reserva Natural Volcan Concepcion</rdfs:label>
    </owl:NamedIndividual>
    


    <!-- http://purl.obolibrary.org/obo/GAZ_00267117 -->

    <owl:NamedIndividual rdf:about="http://purl.obolibrary.org/obo/GAZ_00267117">
        <obo:RO_0001025 rdf:resource="http://purl.obolibrary.org/obo/GAZ_00066800"/>
        <obo:IAO_0000115>A protected area.</obo:IAO_0000115>
        <oboInOwl:hasOBONamespace>GAZ</oboInOwl:hasOBONamespace>
        <oboInOwl:id>GAZ:00267117</oboInOwl:id>
        <rdfs:label>Reserva Natural Cerro Kuskawas</rdfs:label>
    </owl:NamedIndividual>
    


    <!-- http://purl.obolibrary.org/obo/GAZ_00267118 -->

    <owl:NamedIndividual rdf:about="http://purl.obolibrary.org/obo/GAZ_00267118">
        <obo:RO_0001025 rdf:resource="http://purl.obolibrary.org/obo/GAZ_00066800"/>
        <obo:IAO_0000115>A protected area.</obo:IAO_0000115>
        <oboInOwl:hasOBONamespace>GAZ</oboInOwl:hasOBONamespace>
        <oboInOwl:id>GAZ:00267118</oboInOwl:id>
        <rdfs:label>Reserva Natural Salto Rio Yasica</rdfs:label>
    </owl:NamedIndividual>
    


    <!-- http://purl.obolibrary.org/obo/GAZ_00267119 -->

    <owl:NamedIndividual rdf:about="http://purl.obolibrary.org/obo/GAZ_00267119">
        <obo:RO_0001025 rdf:resource="http://purl.obolibrary.org/obo/GAZ_00066800"/>
        <obo:IAO_0000115>A protected area.</obo:IAO_0000115>
        <oboInOwl:hasOBONamespace>GAZ</oboInOwl:hasOBONamespace>
        <oboInOwl:id>GAZ:00267119</oboInOwl:id>
        <rdfs:label>Reserva Natural Cerro Guabule</rdfs:label>
    </owl:NamedIndividual>
    


    <!-- http://purl.obolibrary.org/obo/GAZ_00267120 -->

    <owl:NamedIndividual rdf:about="http://purl.obolibrary.org/obo/GAZ_00267120">
        <obo:RO_0001025 rdf:resource="http://purl.obolibrary.org/obo/GAZ_00066800"/>
        <obo:IAO_0000115>A protected area.</obo:IAO_0000115>
        <oboInOwl:hasOBONamespace>GAZ</oboInOwl:hasOBONamespace>
        <oboInOwl:id>GAZ:00267120</oboInOwl:id>
        <rdfs:label>Reserva Natural Sierra Quirragua</rdfs:label>
    </owl:NamedIndividual>
    


    <!-- http://purl.obolibrary.org/obo/GAZ_00267124 -->

    <owl:NamedIndividual rdf:about="http://purl.obolibrary.org/obo/GAZ_00267124">
        <obo:RO_0001025 rdf:resource="http://purl.obolibrary.org/obo/GAZ_00056214"/>
        <obo:IAO_0000115>A protected area.</obo:IAO_0000115>
        <oboInOwl:hasOBONamespace>GAZ</oboInOwl:hasOBONamespace>
        <oboInOwl:id>GAZ:00267124</oboInOwl:id>
        <rdfs:label>Reserva Natural Cerro Mombachito-La Vieja</rdfs:label>
    </owl:NamedIndividual>
    


    <!-- http://purl.obolibrary.org/obo/GAZ_00267125 -->

    <owl:NamedIndividual rdf:about="http://purl.obolibrary.org/obo/GAZ_00267125">
        <obo:RO_0001025 rdf:resource="http://purl.obolibrary.org/obo/GAZ_00056214"/>
        <obo:IAO_0000115>A protected area.</obo:IAO_0000115>
        <oboInOwl:hasOBONamespace>GAZ</oboInOwl:hasOBONamespace>
        <oboInOwl:id>GAZ:00267125</oboInOwl:id>
        <rdfs:label>Reserva Natural Fila Masigue</rdfs:label>
    </owl:NamedIndividual>
    


    <!-- http://purl.obolibrary.org/obo/GAZ_00267126 -->

    <owl:NamedIndividual rdf:about="http://purl.obolibrary.org/obo/GAZ_00267126">
        <obo:RO_0001025 rdf:resource="http://purl.obolibrary.org/obo/GAZ_00267032"/>
        <obo:IAO_0000115>A protected area.</obo:IAO_0000115>
        <oboInOwl:hasOBONamespace>GAZ</oboInOwl:hasOBONamespace>
        <oboInOwl:id>GAZ:00267126</oboInOwl:id>
        <rdfs:label>Reserva Natural Sierra Amerrisque</rdfs:label>
    </owl:NamedIndividual>
    


    <!-- http://purl.obolibrary.org/obo/GAZ_00267128 -->

    <owl:NamedIndividual rdf:about="http://purl.obolibrary.org/obo/GAZ_00267128">
        <obo:RO_0001025 rdf:resource="http://purl.obolibrary.org/obo/GAZ_00047244"/>
        <obo:IAO_0000115>A protected area.</obo:IAO_0000115>
        <oboInOwl:hasOBONamespace>GAZ</oboInOwl:hasOBONamespace>
        <oboInOwl:id>GAZ:00267128</oboInOwl:id>
        <rdfs:label>Reserva Natural Cerro Alamikamba</rdfs:label>
    </owl:NamedIndividual>
    


    <!-- http://purl.obolibrary.org/obo/GAZ_00267129 -->

    <owl:NamedIndividual rdf:about="http://purl.obolibrary.org/obo/GAZ_00267129">
        <obo:RO_0001025 rdf:resource="http://purl.obolibrary.org/obo/GAZ_00047244"/>
        <obo:IAO_0000115>A protected area.</obo:IAO_0000115>
        <oboInOwl:hasOBONamespace>GAZ</oboInOwl:hasOBONamespace>
        <oboInOwl:id>GAZ:00267129</oboInOwl:id>
        <rdfs:label>Reserva Natural Kligna</rdfs:label>
    </owl:NamedIndividual>
    


    <!-- http://purl.obolibrary.org/obo/GAZ_00267130 -->

    <owl:NamedIndividual rdf:about="http://purl.obolibrary.org/obo/GAZ_00267130">
        <obo:RO_0001025 rdf:resource="http://purl.obolibrary.org/obo/GAZ_00047244"/>
        <obo:IAO_0000115>A protected area.</obo:IAO_0000115>
        <oboInOwl:hasOBONamespace>GAZ</oboInOwl:hasOBONamespace>
        <oboInOwl:id>GAZ:00267130</oboInOwl:id>
        <rdfs:label>Reserva Natural Makantaka</rdfs:label>
    </owl:NamedIndividual>
    


    <!-- http://purl.obolibrary.org/obo/GAZ_00267131 -->

    <owl:NamedIndividual rdf:about="http://purl.obolibrary.org/obo/GAZ_00267131">
        <obo:RO_0001025 rdf:resource="http://purl.obolibrary.org/obo/GAZ_00047244"/>
        <obo:IAO_0000115>A protected area.</obo:IAO_0000115>
        <oboInOwl:hasOBONamespace>GAZ</oboInOwl:hasOBONamespace>
        <oboInOwl:id>GAZ:00267131</oboInOwl:id>
        <rdfs:label>Reserva Natural Limbaika</rdfs:label>
    </owl:NamedIndividual>
    


    <!-- http://purl.obolibrary.org/obo/GAZ_00267132 -->

    <owl:NamedIndividual rdf:about="http://purl.obolibrary.org/obo/GAZ_00267132">
        <obo:RO_0001025 rdf:resource="http://purl.obolibrary.org/obo/GAZ_00047244"/>
        <obo:IAO_0000115>A protected area.</obo:IAO_0000115>
        <oboInOwl:hasOBONamespace>GAZ</oboInOwl:hasOBONamespace>
        <oboInOwl:id>GAZ:00267132</oboInOwl:id>
        <rdfs:label>Reserva Natural Yulu</rdfs:label>
    </owl:NamedIndividual>
    


    <!-- http://purl.obolibrary.org/obo/GAZ_00267133 -->

    <owl:NamedIndividual rdf:about="http://purl.obolibrary.org/obo/GAZ_00267133">
        <obo:RO_0001025 rdf:resource="http://purl.obolibrary.org/obo/GAZ_00047244"/>
        <obo:IAO_0000115>A protected area.</obo:IAO_0000115>
        <oboInOwl:hasOBONamespace>GAZ</oboInOwl:hasOBONamespace>
        <oboInOwl:id>GAZ:00267133</oboInOwl:id>
        <rdfs:label>Reserva Natural Cerro Cola Blanca</rdfs:label>
    </owl:NamedIndividual>
    


    <!-- http://purl.obolibrary.org/obo/GAZ_00267134 -->

    <owl:NamedIndividual rdf:about="http://purl.obolibrary.org/obo/GAZ_00267134">
        <obo:RO_0001025 rdf:resource="http://purl.obolibrary.org/obo/GAZ_00047244"/>
        <obo:IAO_0000115>A protected area.</obo:IAO_0000115>
        <oboInOwl:hasOBONamespace>GAZ</oboInOwl:hasOBONamespace>
        <oboInOwl:id>GAZ:00267134</oboInOwl:id>
        <rdfs:label>Reserva Natural Cerro Bana Cruz</rdfs:label>
    </owl:NamedIndividual>
    


    <!-- http://purl.obolibrary.org/obo/GAZ_00267135 -->

    <owl:NamedIndividual rdf:about="http://purl.obolibrary.org/obo/GAZ_00267135">
        <obo:RO_0001025 rdf:resource="http://purl.obolibrary.org/obo/GAZ_00067069"/>
        <obo:IAO_0000115>A protected area. A Ramsar Site.</obo:IAO_0000115>
        <oboInOwl:hasOBONamespace>GAZ</oboInOwl:hasOBONamespace>
        <oboInOwl:id>GAZ:00267135</oboInOwl:id>
        <rdfs:label>Sitio Ramsar Bahia de Bluefields</rdfs:label>
    </owl:NamedIndividual>
    


    <!-- http://purl.obolibrary.org/obo/GAZ_00267137 -->

    <owl:NamedIndividual rdf:about="http://purl.obolibrary.org/obo/GAZ_00267137">
        <obo:RO_0001025 rdf:resource="http://purl.obolibrary.org/obo/GAZ_00047243"/>
        <obo:IAO_0000115>A protected area.</obo:IAO_0000115>
        <oboInOwl:hasOBONamespace>GAZ</oboInOwl:hasOBONamespace>
        <oboInOwl:id>GAZ:00267137</oboInOwl:id>
        <rdfs:label>Reserva Natural Llanos de Karawala</rdfs:label>
    </owl:NamedIndividual>
    


    <!-- http://purl.obolibrary.org/obo/GAZ_00267138 -->

    <owl:NamedIndividual rdf:about="http://purl.obolibrary.org/obo/GAZ_00267138">
        <obo:RO_0001025 rdf:resource="http://purl.obolibrary.org/obo/GAZ_00067057"/>
        <obo:IAO_0000115>A protected area. A Ramsar Site.</obo:IAO_0000115>
        <oboInOwl:hasOBONamespace>GAZ</oboInOwl:hasOBONamespace>
        <oboInOwl:id>GAZ:00267138</oboInOwl:id>
        <rdfs:label>Sitio Ramsar Humedales de San Miguelito</rdfs:label>
    </owl:NamedIndividual>
    


    <!-- http://purl.obolibrary.org/obo/GAZ_00267139 -->

    <owl:NamedIndividual rdf:about="http://purl.obolibrary.org/obo/GAZ_00267139">
        <obo:RO_0001025 rdf:resource="http://purl.obolibrary.org/obo/GAZ_00066975"/>
        <obo:IAO_0000115>A protected area. A Ramsar Site.</obo:IAO_0000115>
        <oboInOwl:hasOBONamespace>GAZ</oboInOwl:hasOBONamespace>
        <oboInOwl:id>GAZ:00267139</oboInOwl:id>
        <rdfs:label>Sitio Ramsar Apanas-Asturias</rdfs:label>
    </owl:NamedIndividual>
    


    <!-- http://purl.obolibrary.org/obo/GAZ_00267140 -->

    <owl:NamedIndividual rdf:about="http://purl.obolibrary.org/obo/GAZ_00267140">
        <obo:RO_0001025 rdf:resource="http://purl.obolibrary.org/obo/GAZ_00047243"/>
        <obo:IAO_0000115>A river of Nicaragua. Running 430 km from its source near Matagalpa to the Caribbean Sea in the northern part of the Sourthern Atlantic Autonomous Region.</obo:IAO_0000115>
        <oboInOwl:hasOBONamespace>GAZ</oboInOwl:hasOBONamespace>
        <oboInOwl:id>GAZ:00267140</oboInOwl:id>
        <rdfs:label>Rio Grande de Matagalpa</rdfs:label>
    </owl:NamedIndividual>
    


    <!-- http://purl.obolibrary.org/obo/GAZ_00267146 -->

    <owl:NamedIndividual rdf:about="http://purl.obolibrary.org/obo/GAZ_00267146">
        <obo:IAO_0000115>A river.</obo:IAO_0000115>
        <oboInOwl:hasOBONamespace>GAZ</oboInOwl:hasOBONamespace>
        <oboInOwl:id>GAZ:00267146</oboInOwl:id>
        <rdfs:label>Rio Iyas</rdfs:label>
    </owl:NamedIndividual>
    


    <!-- http://purl.obolibrary.org/obo/GAZ_00267147 -->

    <owl:NamedIndividual rdf:about="http://purl.obolibrary.org/obo/GAZ_00267147">
        <obo:RO_0001025 rdf:resource="http://purl.obolibrary.org/obo/GAZ_00047244"/>
        <obo:IAO_0000115>A river.</obo:IAO_0000115>
        <oboInOwl:hasOBONamespace>GAZ</oboInOwl:hasOBONamespace>
        <oboInOwl:id>GAZ:00267147</oboInOwl:id>
        <rdfs:label>Rio Waspuk</rdfs:label>
    </owl:NamedIndividual>
    


    <!-- http://purl.obolibrary.org/obo/GAZ_00267149 -->

    <owl:NamedIndividual rdf:about="http://purl.obolibrary.org/obo/GAZ_00267149">
        <obo:RO_0001025 rdf:resource="http://purl.obolibrary.org/obo/GAZ_00062427"/>
        <obo:IAO_0000115>A river.</obo:IAO_0000115>
        <oboInOwl:hasOBONamespace>GAZ</oboInOwl:hasOBONamespace>
        <oboInOwl:id>GAZ:00267149</oboInOwl:id>
        <rdfs:label>Rio Bocay</rdfs:label>
    </owl:NamedIndividual>
    


    <!-- http://purl.obolibrary.org/obo/GAZ_00267150 -->

    <owl:NamedIndividual rdf:about="http://purl.obolibrary.org/obo/GAZ_00267150">
        <obo:RO_0001025 rdf:resource="http://purl.obolibrary.org/obo/GAZ_00062427"/>
        <obo:IAO_0000115>A river.</obo:IAO_0000115>
        <oboInOwl:hasOBONamespace>GAZ</oboInOwl:hasOBONamespace>
        <oboInOwl:id>GAZ:00267150</oboInOwl:id>
        <rdfs:label>Rio Amaka</rdfs:label>
    </owl:NamedIndividual>
    


    <!-- http://purl.obolibrary.org/obo/GAZ_00267153 -->

    <owl:NamedIndividual rdf:about="http://purl.obolibrary.org/obo/GAZ_00267153">
        <rdf:type rdf:resource="http://purl.obolibrary.org/obo/ENVO_00000098"/>
        <obo:RO_0001025 rdf:resource="http://purl.obolibrary.org/obo/GAZ_00047249"/>
        <obo:IAO_0000115>A cay.</obo:IAO_0000115>
        <oboInOwl:hasOBONamespace>GAZ</oboInOwl:hasOBONamespace>
        <oboInOwl:id>GAZ:00267153</oboInOwl:id>
        <rdfs:label>Cayo Muerto</rdfs:label>
    </owl:NamedIndividual>
    


    <!-- http://purl.obolibrary.org/obo/GAZ_00267154 -->

    <owl:NamedIndividual rdf:about="http://purl.obolibrary.org/obo/GAZ_00267154">
        <obo:RO_0001025 rdf:resource="http://purl.obolibrary.org/obo/GAZ_00047249"/>
        <obo:IAO_0000115>A coral reef.</obo:IAO_0000115>
        <oboInOwl:hasOBONamespace>GAZ</oboInOwl:hasOBONamespace>
        <oboInOwl:id>GAZ:00267154</oboInOwl:id>
        <rdfs:label>London Reef</rdfs:label>
    </owl:NamedIndividual>
    


    <!-- http://purl.obolibrary.org/obo/GAZ_00267155 -->

    <owl:NamedIndividual rdf:about="http://purl.obolibrary.org/obo/GAZ_00267155">
        <rdf:type rdf:resource="http://purl.obolibrary.org/obo/ENVO_00000098"/>
        <obo:RO_0001025 rdf:resource="http://purl.obolibrary.org/obo/GAZ_00047249"/>
        <obo:IAO_0000115>A cay.</obo:IAO_0000115>
        <oboInOwl:hasOBONamespace>GAZ</oboInOwl:hasOBONamespace>
        <oboInOwl:id>GAZ:00267155</oboInOwl:id>
        <rdfs:label>Cayo Londres</rdfs:label>
    </owl:NamedIndividual>
    


    <!-- http://purl.obolibrary.org/obo/GAZ_00267156 -->

    <owl:NamedIndividual rdf:about="http://purl.obolibrary.org/obo/GAZ_00267156">
        <obo:RO_0001025 rdf:resource="http://purl.obolibrary.org/obo/GAZ_00047249"/>
        <obo:IAO_0000115>A coral reef.</obo:IAO_0000115>
        <oboInOwl:hasOBONamespace>GAZ</oboInOwl:hasOBONamespace>
        <oboInOwl:id>GAZ:00267156</oboInOwl:id>
        <rdfs:label>Franklin Reef</rdfs:label>
    </owl:NamedIndividual>
    


    <!-- http://purl.obolibrary.org/obo/GAZ_00267157 -->

    <owl:NamedIndividual rdf:about="http://purl.obolibrary.org/obo/GAZ_00267157">
        <obo:RO_0001025 rdf:resource="http://purl.obolibrary.org/obo/GAZ_00047244"/>
        <obo:IAO_0000115>A river. Drains to the Atlantic Ocean.</obo:IAO_0000115>
        <oboInOwl:hasOBONamespace>GAZ</oboInOwl:hasOBONamespace>
        <oboInOwl:id>GAZ:00267157</oboInOwl:id>
        <rdfs:label>Rio Ulang</rdfs:label>
    </owl:NamedIndividual>
    


    <!-- http://purl.obolibrary.org/obo/GAZ_00267158 -->

    <owl:NamedIndividual rdf:about="http://purl.obolibrary.org/obo/GAZ_00267158">
        <obo:RO_0001025 rdf:resource="http://purl.obolibrary.org/obo/GAZ_00047244"/>
        <obo:IAO_0000115>A river. Drains to the Atlantic Ocean.</obo:IAO_0000115>
        <oboInOwl:hasOBONamespace>GAZ</oboInOwl:hasOBONamespace>
        <oboInOwl:id>GAZ:00267158</oboInOwl:id>
        <rdfs:label>Rio Wawa</rdfs:label>
    </owl:NamedIndividual>
    


    <!-- http://purl.obolibrary.org/obo/GAZ_00267161 -->

    <owl:NamedIndividual rdf:about="http://purl.obolibrary.org/obo/GAZ_00267161">
        <obo:RO_0001025 rdf:resource="http://purl.obolibrary.org/obo/GAZ_00047244"/>
        <obo:IAO_0000115>A river. Drains to the Atlantic Ocean at Laguna Wounta.</obo:IAO_0000115>
        <oboInOwl:hasOBONamespace>GAZ</oboInOwl:hasOBONamespace>
        <oboInOwl:id>GAZ:00267161</oboInOwl:id>
        <rdfs:label>Rio Kukalaya</rdfs:label>
    </owl:NamedIndividual>
    


    <!-- http://purl.obolibrary.org/obo/GAZ_00267163 -->

    <owl:NamedIndividual rdf:about="http://purl.obolibrary.org/obo/GAZ_00267163">
        <obo:RO_0001025 rdf:resource="http://purl.obolibrary.org/obo/GAZ_00047244"/>
        <obo:IAO_0000115>A river.</obo:IAO_0000115>
        <oboInOwl:hasOBONamespace>GAZ</oboInOwl:hasOBONamespace>
        <oboInOwl:id>GAZ:00267163</oboInOwl:id>
        <rdfs:label>Rio Prinzapolka</rdfs:label>
    </owl:NamedIndividual>
    


    <!-- http://purl.obolibrary.org/obo/GAZ_00267164 -->

    <owl:NamedIndividual rdf:about="http://purl.obolibrary.org/obo/GAZ_00267164">
        <obo:RO_0001025 rdf:resource="http://purl.obolibrary.org/obo/GAZ_00047244"/>
        <obo:IAO_0000115>A river.</obo:IAO_0000115>
        <oboInOwl:hasOBONamespace>GAZ</oboInOwl:hasOBONamespace>
        <oboInOwl:id>GAZ:00267164</oboInOwl:id>
        <rdfs:label>Rio Bambana</rdfs:label>
    </owl:NamedIndividual>
    


    <!-- http://purl.obolibrary.org/obo/GAZ_00267167 -->

    <owl:NamedIndividual rdf:about="http://purl.obolibrary.org/obo/GAZ_00267167">
        <obo:RO_0001025 rdf:resource="http://purl.obolibrary.org/obo/GAZ_00047244"/>
        <obo:IAO_0000115>A river.</obo:IAO_0000115>
        <oboInOwl:hasOBONamespace>GAZ</oboInOwl:hasOBONamespace>
        <oboInOwl:id>GAZ:00267167</oboInOwl:id>
        <rdfs:label>Rio Yaoya</rdfs:label>
    </owl:NamedIndividual>
    


    <!-- http://purl.obolibrary.org/obo/GAZ_00267168 -->

    <owl:NamedIndividual rdf:about="http://purl.obolibrary.org/obo/GAZ_00267168">
        <obo:RO_0001025 rdf:resource="http://purl.obolibrary.org/obo/GAZ_00047244"/>
        <obo:IAO_0000115>A coastal lagoon.</obo:IAO_0000115>
        <oboInOwl:hasOBONamespace>GAZ</oboInOwl:hasOBONamespace>
        <oboInOwl:id>GAZ:00267168</oboInOwl:id>
        <rdfs:label>Laguna Gracias a Dos</rdfs:label>
    </owl:NamedIndividual>
    


    <!-- http://purl.obolibrary.org/obo/GAZ_00267169 -->

    <owl:NamedIndividual rdf:about="http://purl.obolibrary.org/obo/GAZ_00267169">
        <obo:RO_0001025 rdf:resource="http://purl.obolibrary.org/obo/GAZ_00047244"/>
        <obo:IAO_0000115>A coastal lagoon.</obo:IAO_0000115>
        <oboInOwl:hasOBONamespace>GAZ</oboInOwl:hasOBONamespace>
        <oboInOwl:id>GAZ:00267169</oboInOwl:id>
        <rdfs:label>Laguna Bismuna</rdfs:label>
    </owl:NamedIndividual>
    


    <!-- http://purl.obolibrary.org/obo/GAZ_00267170 -->

    <owl:NamedIndividual rdf:about="http://purl.obolibrary.org/obo/GAZ_00267170">
        <obo:RO_0001025 rdf:resource="http://purl.obolibrary.org/obo/GAZ_00047244"/>
        <obo:IAO_0000115>A coastal lagoon.</obo:IAO_0000115>
        <oboInOwl:hasOBONamespace>GAZ</oboInOwl:hasOBONamespace>
        <oboInOwl:id>GAZ:00267170</oboInOwl:id>
        <rdfs:label>Laguna Sikapakia</rdfs:label>
    </owl:NamedIndividual>
    


    <!-- http://purl.obolibrary.org/obo/GAZ_00267171 -->

    <owl:NamedIndividual rdf:about="http://purl.obolibrary.org/obo/GAZ_00267171">
        <obo:RO_0001025 rdf:resource="http://purl.obolibrary.org/obo/GAZ_00047244"/>
        <obo:IAO_0000115>A coastal lagoon.</obo:IAO_0000115>
        <oboInOwl:hasOBONamespace>GAZ</oboInOwl:hasOBONamespace>
        <oboInOwl:id>GAZ:00267171</oboInOwl:id>
        <rdfs:label>Laguna Li-Dakura</rdfs:label>
    </owl:NamedIndividual>
    


    <!-- http://purl.obolibrary.org/obo/GAZ_00267172 -->

    <owl:NamedIndividual rdf:about="http://purl.obolibrary.org/obo/GAZ_00267172">
        <obo:RO_0001025 rdf:resource="http://purl.obolibrary.org/obo/GAZ_00047244"/>
        <obo:IAO_0000115>A coastal lagoon.</obo:IAO_0000115>
        <oboInOwl:hasOBONamespace>GAZ</oboInOwl:hasOBONamespace>
        <oboInOwl:id>GAZ:00267172</oboInOwl:id>
        <rdfs:label>Laguna Dakura</rdfs:label>
    </owl:NamedIndividual>
    


    <!-- http://purl.obolibrary.org/obo/GAZ_00267173 -->

    <owl:NamedIndividual rdf:about="http://purl.obolibrary.org/obo/GAZ_00267173">
        <obo:RO_0001025 rdf:resource="http://purl.obolibrary.org/obo/GAZ_00047244"/>
        <obo:IAO_0000115>A coastal lagoon.</obo:IAO_0000115>
        <oboInOwl:hasOBONamespace>GAZ</oboInOwl:hasOBONamespace>
        <oboInOwl:id>GAZ:00267173</oboInOwl:id>
        <rdfs:label>Laguna Pahara</rdfs:label>
    </owl:NamedIndividual>
    


    <!-- http://purl.obolibrary.org/obo/GAZ_00267174 -->

    <owl:NamedIndividual rdf:about="http://purl.obolibrary.org/obo/GAZ_00267174">
        <obo:RO_0001025 rdf:resource="http://purl.obolibrary.org/obo/GAZ_00047244"/>
        <obo:IAO_0000115>A coastal lagoon.</obo:IAO_0000115>
        <oboInOwl:hasOBONamespace>GAZ</oboInOwl:hasOBONamespace>
        <oboInOwl:id>GAZ:00267174</oboInOwl:id>
        <rdfs:label>Laguna Karata</rdfs:label>
    </owl:NamedIndividual>
    


    <!-- http://purl.obolibrary.org/obo/GAZ_00267175 -->

    <owl:NamedIndividual rdf:about="http://purl.obolibrary.org/obo/GAZ_00267175">
        <obo:RO_0001025 rdf:resource="http://purl.obolibrary.org/obo/GAZ_00047244"/>
        <obo:IAO_0000115>A coastal lagoon.</obo:IAO_0000115>
        <oboInOwl:hasOBONamespace>GAZ</oboInOwl:hasOBONamespace>
        <oboInOwl:id>GAZ:00267175</oboInOwl:id>
        <rdfs:label>Laguna Wankamaya</rdfs:label>
    </owl:NamedIndividual>
    


    <!-- http://purl.obolibrary.org/obo/GAZ_00267176 -->

    <owl:NamedIndividual rdf:about="http://purl.obolibrary.org/obo/GAZ_00267176">
        <obo:RO_0001025 rdf:resource="http://purl.obolibrary.org/obo/GAZ_00047244"/>
        <obo:IAO_0000115>A coastal lagoon.</obo:IAO_0000115>
        <oboInOwl:hasOBONamespace>GAZ</oboInOwl:hasOBONamespace>
        <oboInOwl:id>GAZ:00267176</oboInOwl:id>
        <rdfs:label>Laguna Wounta</rdfs:label>
    </owl:NamedIndividual>
    


    <!-- http://purl.obolibrary.org/obo/GAZ_00267177 -->

    <owl:NamedIndividual rdf:about="http://purl.obolibrary.org/obo/GAZ_00267177">
        <obo:RO_0001025 rdf:resource="http://purl.obolibrary.org/obo/GAZ_00047243"/>
        <obo:IAO_0000115>A river. Discharges to the Atlantic Ocean.</obo:IAO_0000115>
        <oboInOwl:hasOBONamespace>GAZ</oboInOwl:hasOBONamespace>
        <oboInOwl:id>GAZ:00267177</oboInOwl:id>
        <rdfs:label>Rio Kurinwas</rdfs:label>
    </owl:NamedIndividual>
    


    <!-- http://purl.obolibrary.org/obo/GAZ_00267178 -->

    <owl:NamedIndividual rdf:about="http://purl.obolibrary.org/obo/GAZ_00267178">
        <obo:RO_0001025 rdf:resource="http://purl.obolibrary.org/obo/GAZ_00047243"/>
        <obo:IAO_0000115>A river. Discharges to the Atlantic Ocean.</obo:IAO_0000115>
        <oboInOwl:hasOBONamespace>GAZ</oboInOwl:hasOBONamespace>
        <oboInOwl:id>GAZ:00267178</oboInOwl:id>
        <rdfs:label>Rio Wawasang</rdfs:label>
    </owl:NamedIndividual>
    


    <!-- http://purl.obolibrary.org/obo/GAZ_00267179 -->

    <owl:NamedIndividual rdf:about="http://purl.obolibrary.org/obo/GAZ_00267179">
        <obo:RO_0001025 rdf:resource="http://purl.obolibrary.org/obo/GAZ_00047243"/>
        <obo:IAO_0000115>A river. Discharges to the Atlantic Ocean.</obo:IAO_0000115>
        <oboInOwl:hasOBONamespace>GAZ</oboInOwl:hasOBONamespace>
        <oboInOwl:id>GAZ:00267179</oboInOwl:id>
        <rdfs:label>Rio Escondido</rdfs:label>
    </owl:NamedIndividual>
    


    <!-- http://purl.obolibrary.org/obo/GAZ_00267180 -->

    <owl:NamedIndividual rdf:about="http://purl.obolibrary.org/obo/GAZ_00267180">
        <obo:RO_0001025 rdf:resource="http://purl.obolibrary.org/obo/GAZ_00047243"/>
        <obo:IAO_0000115>A river.</obo:IAO_0000115>
        <oboInOwl:hasOBONamespace>GAZ</oboInOwl:hasOBONamespace>
        <oboInOwl:id>GAZ:00267180</oboInOwl:id>
        <rdfs:label>Rio Kama</rdfs:label>
    </owl:NamedIndividual>
    


    <!-- http://purl.obolibrary.org/obo/GAZ_00267183 -->

    <owl:NamedIndividual rdf:about="http://purl.obolibrary.org/obo/GAZ_00267183">
        <obo:RO_0001025 rdf:resource="http://purl.obolibrary.org/obo/GAZ_00047243"/>
        <obo:IAO_0000115>A river.</obo:IAO_0000115>
        <oboInOwl:hasOBONamespace>GAZ</oboInOwl:hasOBONamespace>
        <oboInOwl:id>GAZ:00267183</oboInOwl:id>
        <rdfs:label>Rio Plata</rdfs:label>
    </owl:NamedIndividual>
    


    <!-- http://purl.obolibrary.org/obo/GAZ_00267186 -->

    <owl:NamedIndividual rdf:about="http://purl.obolibrary.org/obo/GAZ_00267186">
        <obo:RO_0001025 rdf:resource="http://purl.obolibrary.org/obo/GAZ_00047243"/>
        <obo:IAO_0000115>A river. Discharges to Bahia de Bluefields.</obo:IAO_0000115>
        <oboInOwl:hasOBONamespace>GAZ</oboInOwl:hasOBONamespace>
        <oboInOwl:id>GAZ:00267186</oboInOwl:id>
        <rdfs:label>Rio Kukra</rdfs:label>
    </owl:NamedIndividual>
    


    <!-- http://purl.obolibrary.org/obo/GAZ_00267187 -->

    <owl:NamedIndividual rdf:about="http://purl.obolibrary.org/obo/GAZ_00267187">
        <obo:RO_0001025 rdf:resource="http://purl.obolibrary.org/obo/GAZ_00047243"/>
        <obo:IAO_0000115>A river. Discharges to the Atlantic Ocean.</obo:IAO_0000115>
        <oboInOwl:hasOBONamespace>GAZ</oboInOwl:hasOBONamespace>
        <oboInOwl:id>GAZ:00267187</oboInOwl:id>
        <rdfs:label>Rio Punta Gorda</rdfs:label>
    </owl:NamedIndividual>
    


    <!-- http://purl.obolibrary.org/obo/GAZ_00267188 -->

    <owl:NamedIndividual rdf:about="http://purl.obolibrary.org/obo/GAZ_00267188">
        <obo:RO_0001025 rdf:resource="http://purl.obolibrary.org/obo/GAZ_00047243"/>
        <obo:IAO_0000115>A river. Discharges to Bahia Punta Gorda.</obo:IAO_0000115>
        <oboInOwl:hasOBONamespace>GAZ</oboInOwl:hasOBONamespace>
        <oboInOwl:id>GAZ:00267188</oboInOwl:id>
        <rdfs:label>Rio Maiz</rdfs:label>
    </owl:NamedIndividual>
    


    <!-- http://purl.obolibrary.org/obo/GAZ_00267190 -->

    <owl:NamedIndividual rdf:about="http://purl.obolibrary.org/obo/GAZ_00267190">
        <obo:RO_0001025 rdf:resource="http://purl.obolibrary.org/obo/GAZ_00047243"/>
        <obo:IAO_0000115>A coastal lagoon.</obo:IAO_0000115>
        <oboInOwl:hasOBONamespace>GAZ</oboInOwl:hasOBONamespace>
        <oboInOwl:id>GAZ:00267190</oboInOwl:id>
        <rdfs:label>Laguna Top Lock</rdfs:label>
    </owl:NamedIndividual>
    


    <!-- http://purl.obolibrary.org/obo/GAZ_00267191 -->

    <owl:NamedIndividual rdf:about="http://purl.obolibrary.org/obo/GAZ_00267191">
        <obo:RO_0001025 rdf:resource="http://purl.obolibrary.org/obo/GAZ_00047243"/>
        <obo:IAO_0000115>A coastal lagoon.</obo:IAO_0000115>
        <oboInOwl:hasOBONamespace>GAZ</oboInOwl:hasOBONamespace>
        <oboInOwl:id>GAZ:00267191</oboInOwl:id>
        <rdfs:label>Laguna Grande</rdfs:label>
    </owl:NamedIndividual>
    


    <!-- http://purl.obolibrary.org/obo/GAZ_00267192 -->

    <owl:NamedIndividual rdf:about="http://purl.obolibrary.org/obo/GAZ_00267192">
        <obo:RO_0001025 rdf:resource="http://purl.obolibrary.org/obo/GAZ_00047243"/>
        <obo:IAO_0000115>A coastal lagoon.</obo:IAO_0000115>
        <oboInOwl:hasOBONamespace>GAZ</oboInOwl:hasOBONamespace>
        <oboInOwl:id>GAZ:00267192</oboInOwl:id>
        <rdfs:label>Laguna Sonie</rdfs:label>
    </owl:NamedIndividual>
    


    <!-- http://purl.obolibrary.org/obo/GAZ_00267193 -->

    <owl:NamedIndividual rdf:about="http://purl.obolibrary.org/obo/GAZ_00267193">
        <obo:RO_0001025 rdf:resource="http://purl.obolibrary.org/obo/GAZ_00047243"/>
        <obo:IAO_0000115>A coastal lagoon.</obo:IAO_0000115>
        <oboInOwl:hasOBONamespace>GAZ</oboInOwl:hasOBONamespace>
        <oboInOwl:id>GAZ:00267193</oboInOwl:id>
        <rdfs:label>Laguna Smokey Lane</rdfs:label>
    </owl:NamedIndividual>
    


    <!-- http://purl.obolibrary.org/obo/GAZ_00267194 -->

    <owl:NamedIndividual rdf:about="http://purl.obolibrary.org/obo/GAZ_00267194">
        <obo:RO_0001025 rdf:resource="http://purl.obolibrary.org/obo/GAZ_00047243"/>
        <obo:IAO_0000115>A large bay.</obo:IAO_0000115>
        <oboInOwl:hasOBONamespace>GAZ</oboInOwl:hasOBONamespace>
        <oboInOwl:id>GAZ:00267194</oboInOwl:id>
        <rdfs:label>Bahia de Perlas</rdfs:label>
    </owl:NamedIndividual>
    


    <!-- http://purl.obolibrary.org/obo/GAZ_00267195 -->

    <owl:NamedIndividual rdf:about="http://purl.obolibrary.org/obo/GAZ_00267195">
        <obo:RO_0001025 rdf:resource="http://purl.obolibrary.org/obo/GAZ_00047243"/>
        <obo:IAO_0000115>A bay protected from the open sea by Isa del Venado.</obo:IAO_0000115>
        <oboInOwl:hasOBONamespace>GAZ</oboInOwl:hasOBONamespace>
        <oboInOwl:id>GAZ:00267195</oboInOwl:id>
        <rdfs:label>Bahia de Bluefields</rdfs:label>
    </owl:NamedIndividual>
    


    <!-- http://purl.obolibrary.org/obo/GAZ_00267196 -->

    <owl:NamedIndividual rdf:about="http://purl.obolibrary.org/obo/GAZ_00267196">
        <obo:IAO_0000115>A shallow coastal bay.</obo:IAO_0000115>
        <oboInOwl:hasOBONamespace>GAZ</oboInOwl:hasOBONamespace>
        <oboInOwl:id>GAZ:00267196</oboInOwl:id>
        <rdfs:label>Bahia Punta Gorda</rdfs:label>
    </owl:NamedIndividual>
    


    <!-- http://purl.obolibrary.org/obo/GAZ_00267197 -->

    <owl:NamedIndividual rdf:about="http://purl.obolibrary.org/obo/GAZ_00267197">
        <obo:RO_0001025 rdf:resource="http://purl.obolibrary.org/obo/GAZ_00047261"/>
        <obo:IAO_0000115>A shallow coastal bay.</obo:IAO_0000115>
        <oboInOwl:hasOBONamespace>GAZ</oboInOwl:hasOBONamespace>
        <oboInOwl:id>GAZ:00267197</oboInOwl:id>
        <rdfs:label>Bahia de San Juan del Norte</rdfs:label>
    </owl:NamedIndividual>
    


    <!-- http://purl.obolibrary.org/obo/GAZ_00267198 -->

    <owl:NamedIndividual rdf:about="http://purl.obolibrary.org/obo/GAZ_00267198">
        <obo:RO_0001025 rdf:resource="http://purl.obolibrary.org/obo/GAZ_00047243"/>
        <obo:IAO_0000115>A coastal island between Bahia de Bluefields and the sea.</obo:IAO_0000115>
        <oboInOwl:hasOBONamespace>GAZ</oboInOwl:hasOBONamespace>
        <oboInOwl:id>GAZ:00267198</oboInOwl:id>
        <rdfs:label>Isla del Venado</rdfs:label>
    </owl:NamedIndividual>
    


    <!-- http://purl.obolibrary.org/obo/GAZ_00267199 -->

    <owl:NamedIndividual rdf:about="http://purl.obolibrary.org/obo/GAZ_00267199">
        <obo:RO_0001025 rdf:resource="http://purl.obolibrary.org/obo/GAZ_00047243"/>
        <obo:IAO_0000115>An offshore island. Located SW of Bluefields, S of Isla del Venado and N of Monkey Point.</obo:IAO_0000115>
        <oboInOwl:hasOBONamespace>GAZ</oboInOwl:hasOBONamespace>
        <oboInOwl:id>GAZ:00267199</oboInOwl:id>
        <rdfs:label>Cayo Guano</rdfs:label>
    </owl:NamedIndividual>
    


    <!-- http://purl.obolibrary.org/obo/GAZ_00267200 -->

    <owl:NamedIndividual rdf:about="http://purl.obolibrary.org/obo/GAZ_00267200">
        <obo:RO_0001025 rdf:resource="http://purl.obolibrary.org/obo/GAZ_00047243"/>
        <obo:IAO_0000115>An offshore island. Located SW of Bluefields, S of Isla del Venado and N of Monkey Point.</obo:IAO_0000115>
        <oboInOwl:hasOBONamespace>GAZ</oboInOwl:hasOBONamespace>
        <oboInOwl:id>GAZ:00267200</oboInOwl:id>
        <rdfs:label>Cayo Pigeon</rdfs:label>
    </owl:NamedIndividual>
    


    <!-- http://purl.obolibrary.org/obo/GAZ_00267201 -->

    <owl:NamedIndividual rdf:about="http://purl.obolibrary.org/obo/GAZ_00267201">
        <obo:RO_0001025 rdf:resource="http://purl.obolibrary.org/obo/GAZ_00047243"/>
        <obo:IAO_0000115>An offshore island. Located SW of Bluefields, S of Isla del Venado and N of Monkey Point.</obo:IAO_0000115>
        <oboInOwl:hasOBONamespace>GAZ</oboInOwl:hasOBONamespace>
        <oboInOwl:id>GAZ:00267201</oboInOwl:id>
        <rdfs:label>Cayo French Man</rdfs:label>
    </owl:NamedIndividual>
    


    <!-- http://purl.obolibrary.org/obo/GAZ_00267202 -->

    <owl:NamedIndividual rdf:about="http://purl.obolibrary.org/obo/GAZ_00267202">
        <obo:RO_0001025 rdf:resource="http://purl.obolibrary.org/obo/GAZ_00047243"/>
        <obo:IAO_0000115>A river.</obo:IAO_0000115>
        <oboInOwl:hasOBONamespace>GAZ</oboInOwl:hasOBONamespace>
        <oboInOwl:id>GAZ:00267202</oboInOwl:id>
        <rdfs:label>Rio Iquinis</rdfs:label>
    </owl:NamedIndividual>
    


    <!-- http://purl.obolibrary.org/obo/GAZ_00267203 -->

    <owl:NamedIndividual rdf:about="http://purl.obolibrary.org/obo/GAZ_00267203">
        <obo:RO_0001025 rdf:resource="http://purl.obolibrary.org/obo/GAZ_00047243"/>
        <obo:IAO_0000115>A river.</obo:IAO_0000115>
        <oboInOwl:hasOBONamespace>GAZ</oboInOwl:hasOBONamespace>
        <oboInOwl:id>GAZ:00267203</oboInOwl:id>
        <rdfs:label>Cano Negro</rdfs:label>
    </owl:NamedIndividual>
    


    <!-- http://purl.obolibrary.org/obo/GAZ_00267207 -->

    <owl:NamedIndividual rdf:about="http://purl.obolibrary.org/obo/GAZ_00267207">
        <obo:RO_0001025 rdf:resource="http://purl.obolibrary.org/obo/GAZ_00047261"/>
        <obo:IAO_0000115>A river.</obo:IAO_0000115>
        <oboInOwl:hasOBONamespace>GAZ</oboInOwl:hasOBONamespace>
        <oboInOwl:id>GAZ:00267207</oboInOwl:id>
        <rdfs:label>Rio Sabo Jose</rdfs:label>
    </owl:NamedIndividual>
    


    <!-- http://purl.obolibrary.org/obo/GAZ_00267208 -->

    <owl:NamedIndividual rdf:about="http://purl.obolibrary.org/obo/GAZ_00267208">
        <obo:RO_0001025 rdf:resource="http://purl.obolibrary.org/obo/GAZ_00047261"/>
        <obo:IAO_0000115>A river.</obo:IAO_0000115>
        <oboInOwl:hasOBONamespace>GAZ</oboInOwl:hasOBONamespace>
        <oboInOwl:id>GAZ:00267208</oboInOwl:id>
        <rdfs:label>Rio Santa Cruz</rdfs:label>
    </owl:NamedIndividual>
    


    <!-- http://purl.obolibrary.org/obo/GAZ_00267209 -->

    <owl:NamedIndividual rdf:about="http://purl.obolibrary.org/obo/GAZ_00267209">
        <obo:RO_0001025 rdf:resource="http://purl.obolibrary.org/obo/GAZ_00047258"/>
        <obo:IAO_0000115>An island.</obo:IAO_0000115>
        <oboInOwl:hasOBONamespace>GAZ</oboInOwl:hasOBONamespace>
        <oboInOwl:id>GAZ:00267209</oboInOwl:id>
        <rdfs:label>Isla El Zapote</rdfs:label>
    </owl:NamedIndividual>
    


    <!-- http://purl.obolibrary.org/obo/GAZ_00267210 -->

    <owl:NamedIndividual rdf:about="http://purl.obolibrary.org/obo/GAZ_00267210">
        <obo:RO_0001025 rdf:resource="http://purl.obolibrary.org/obo/GAZ_00047258"/>
        <obo:IAO_0000115>An island.</obo:IAO_0000115>
        <oboInOwl:hasOBONamespace>GAZ</oboInOwl:hasOBONamespace>
        <oboInOwl:id>GAZ:00267210</oboInOwl:id>
        <rdfs:label>Isla Chichicaste</rdfs:label>
    </owl:NamedIndividual>
    


    <!-- http://purl.obolibrary.org/obo/GAZ_00267212 -->

    <owl:NamedIndividual rdf:about="http://purl.obolibrary.org/obo/GAZ_00267212">
        <obo:RO_0001025 rdf:resource="http://purl.obolibrary.org/obo/GAZ_00047261"/>
        <obo:IAO_0000115>A river.</obo:IAO_0000115>
        <oboInOwl:hasOBONamespace>GAZ</oboInOwl:hasOBONamespace>
        <oboInOwl:id>GAZ:00267212</oboInOwl:id>
        <rdfs:label>Rio Canastro</rdfs:label>
    </owl:NamedIndividual>
    


    <!-- http://purl.obolibrary.org/obo/GAZ_00267213 -->

    <owl:NamedIndividual rdf:about="http://purl.obolibrary.org/obo/GAZ_00267213">
        <obo:RO_0001025 rdf:resource="http://purl.obolibrary.org/obo/GAZ_00047261"/>
        <obo:IAO_0000115>A river.</obo:IAO_0000115>
        <oboInOwl:hasOBONamespace>GAZ</oboInOwl:hasOBONamespace>
        <oboInOwl:id>GAZ:00267213</oboInOwl:id>
        <rdfs:label>Rio Tute</rdfs:label>
    </owl:NamedIndividual>
    


    <!-- http://purl.obolibrary.org/obo/GAZ_00267214 -->

    <owl:NamedIndividual rdf:about="http://purl.obolibrary.org/obo/GAZ_00267214">
        <obo:RO_0001025 rdf:resource="http://purl.obolibrary.org/obo/GAZ_00047261"/>
        <obo:IAO_0000115>A river.</obo:IAO_0000115>
        <oboInOwl:hasOBONamespace>GAZ</oboInOwl:hasOBONamespace>
        <oboInOwl:id>GAZ:00267214</oboInOwl:id>
        <rdfs:label>Rio Tepenaguasapa</rdfs:label>
    </owl:NamedIndividual>
    


    <!-- http://purl.obolibrary.org/obo/GAZ_00267215 -->

    <owl:NamedIndividual rdf:about="http://purl.obolibrary.org/obo/GAZ_00267215">
        <obo:RO_0001025 rdf:resource="http://purl.obolibrary.org/obo/GAZ_00047261"/>
        <obo:IAO_0000115>Islands.</obo:IAO_0000115>
        <oboInOwl:hasOBONamespace>GAZ</oboInOwl:hasOBONamespace>
        <oboInOwl:id>GAZ:00267215</oboInOwl:id>
        <rdfs:label>Islas San Bernardo</rdfs:label>
    </owl:NamedIndividual>
    


    <!-- http://purl.obolibrary.org/obo/GAZ_00267216 -->

    <owl:NamedIndividual rdf:about="http://purl.obolibrary.org/obo/GAZ_00267216">
        <obo:RO_0001025 rdf:resource="http://purl.obolibrary.org/obo/GAZ_00066798"/>
        <obo:IAO_0000115>Islands.</obo:IAO_0000115>
        <oboInOwl:hasOBONamespace>GAZ</oboInOwl:hasOBONamespace>
        <oboInOwl:id>GAZ:00267216</oboInOwl:id>
        <rdfs:label>Islas El Nancital</rdfs:label>
    </owl:NamedIndividual>
    


    <!-- http://purl.obolibrary.org/obo/GAZ_00267217 -->

    <owl:NamedIndividual rdf:about="http://purl.obolibrary.org/obo/GAZ_00267217">
        <obo:RO_0001025 rdf:resource="http://purl.obolibrary.org/obo/GAZ_00066798"/>
        <obo:IAO_0000115>An island.</obo:IAO_0000115>
        <oboInOwl:hasOBONamespace>GAZ</oboInOwl:hasOBONamespace>
        <oboInOwl:id>GAZ:00267217</oboInOwl:id>
        <rdfs:label>Isla Grande</rdfs:label>
    </owl:NamedIndividual>
    


    <!-- http://purl.obolibrary.org/obo/GAZ_00267218 -->

    <owl:NamedIndividual rdf:about="http://purl.obolibrary.org/obo/GAZ_00267218">
        <obo:RO_0001025 rdf:resource="http://purl.obolibrary.org/obo/GAZ_00066798"/>
        <obo:IAO_0000115>An island.</obo:IAO_0000115>
        <oboInOwl:hasOBONamespace>GAZ</oboInOwl:hasOBONamespace>
        <oboInOwl:id>GAZ:00267218</oboInOwl:id>
        <rdfs:label>Isla Redonda</rdfs:label>
    </owl:NamedIndividual>
    


    <!-- http://purl.obolibrary.org/obo/GAZ_00267219 -->

    <owl:NamedIndividual rdf:about="http://purl.obolibrary.org/obo/GAZ_00267219">
        <obo:RO_0001025 rdf:resource="http://purl.obolibrary.org/obo/GAZ_00066798"/>
        <obo:IAO_0000115>An island.</obo:IAO_0000115>
        <oboInOwl:hasOBONamespace>GAZ</oboInOwl:hasOBONamespace>
        <oboInOwl:id>GAZ:00267219</oboInOwl:id>
        <rdfs:label>Isla Muerto</rdfs:label>
    </owl:NamedIndividual>
    


    <!-- http://purl.obolibrary.org/obo/GAZ_00267220 -->

    <owl:NamedIndividual rdf:about="http://purl.obolibrary.org/obo/GAZ_00267220">
        <obo:RO_0001025 rdf:resource="http://purl.obolibrary.org/obo/GAZ_00066798"/>
        <obo:IAO_0000115>A river.</obo:IAO_0000115>
        <oboInOwl:hasOBONamespace>GAZ</oboInOwl:hasOBONamespace>
        <oboInOwl:id>GAZ:00267220</oboInOwl:id>
        <rdfs:label>Rio Ojecuapa</rdfs:label>
    </owl:NamedIndividual>
    


    <!-- http://purl.obolibrary.org/obo/GAZ_00267221 -->

    <owl:NamedIndividual rdf:about="http://purl.obolibrary.org/obo/GAZ_00267221">
        <obo:RO_0001025 rdf:resource="http://purl.obolibrary.org/obo/GAZ_00066798"/>
        <obo:IAO_0000115>A river.</obo:IAO_0000115>
        <oboInOwl:hasOBONamespace>GAZ</oboInOwl:hasOBONamespace>
        <oboInOwl:id>GAZ:00267221</oboInOwl:id>
        <rdfs:label>Rio Cuisala</rdfs:label>
    </owl:NamedIndividual>
    


    <!-- http://purl.obolibrary.org/obo/GAZ_00267224 -->

    <owl:NamedIndividual rdf:about="http://purl.obolibrary.org/obo/GAZ_00267224">
        <obo:RO_0001025 rdf:resource="http://purl.obolibrary.org/obo/GAZ_00056204"/>
        <obo:IAO_0000115>An island where Rio Tipitapa discharges into Lake Nicaragua.</obo:IAO_0000115>
        <oboInOwl:hasOBONamespace>GAZ</oboInOwl:hasOBONamespace>
        <oboInOwl:id>GAZ:00267224</oboInOwl:id>
        <rdfs:label>Isla Las Calabazas</rdfs:label>
    </owl:NamedIndividual>
    


    <!-- http://purl.obolibrary.org/obo/GAZ_00267227 -->

    <owl:NamedIndividual rdf:about="http://purl.obolibrary.org/obo/GAZ_00267227">
        <obo:RO_0001025 rdf:resource="http://purl.obolibrary.org/obo/GAZ_00056208"/>
        <obo:IAO_0000115>A lagoon on the shore of Lake Nicaragua.</obo:IAO_0000115>
        <oboInOwl:hasOBONamespace>GAZ</oboInOwl:hasOBONamespace>
        <oboInOwl:id>GAZ:00267227</oboInOwl:id>
        <rdfs:label>Laguna Nocarime</rdfs:label>
    </owl:NamedIndividual>
    


    <!-- http://purl.obolibrary.org/obo/GAZ_00267229 -->

    <owl:NamedIndividual rdf:about="http://purl.obolibrary.org/obo/GAZ_00267229">
        <obo:RO_0001025 rdf:resource="http://purl.obolibrary.org/obo/GAZ_00066799"/>
        <obo:IAO_0000115>A river. Discharges to the Pacific Ocean.</obo:IAO_0000115>
        <oboInOwl:hasOBONamespace>GAZ</oboInOwl:hasOBONamespace>
        <oboInOwl:id>GAZ:00267229</oboInOwl:id>
        <rdfs:label>Rio Casares</rdfs:label>
    </owl:NamedIndividual>
    


    <!-- http://purl.obolibrary.org/obo/GAZ_00267231 -->

    <owl:NamedIndividual rdf:about="http://purl.obolibrary.org/obo/GAZ_00267231">
        <obo:RO_0001025 rdf:resource="http://purl.obolibrary.org/obo/GAZ_00005219"/>
        <obo:IAO_0000115>A river. Discharges to the Gulf of Fonseca.</obo:IAO_0000115>
        <oboInOwl:hasOBONamespace>GAZ</oboInOwl:hasOBONamespace>
        <oboInOwl:id>GAZ:00267231</oboInOwl:id>
        <rdfs:label>Rio Estro Real</rdfs:label>
    </owl:NamedIndividual>
    


    <!-- http://purl.obolibrary.org/obo/GAZ_00267234 -->

    <owl:NamedIndividual rdf:about="http://purl.obolibrary.org/obo/GAZ_00267234">
        <obo:RO_0001025 rdf:resource="http://purl.obolibrary.org/obo/GAZ_00056193"/>
        <obo:IAO_0000115>A river.</obo:IAO_0000115>
        <oboInOwl:hasOBONamespace>GAZ</oboInOwl:hasOBONamespace>
        <oboInOwl:id>GAZ:00267234</oboInOwl:id>
        <rdfs:label>Rio Sinecapa</rdfs:label>
    </owl:NamedIndividual>
    


    <!-- 
    ///////////////////////////////////////////////////////////////////////////////////////
    //
    // Annotations
    //
    ///////////////////////////////////////////////////////////////////////////////////////
     -->

    <rdf:Description rdf:about="http://purl.obolibrary.org/obo/GAZ_00000094">
        <oboInOwl:hasOBONamespace>GAZ</oboInOwl:hasOBONamespace>
        <oboInOwl:id>GAZ:00000094</oboInOwl:id>
        <rdfs:label>Cayanlipe</rdfs:label>
    </rdf:Description>
    <rdf:Description rdf:about="http://purl.obolibrary.org/obo/GAZ_00005218">
        <oboInOwl:id>GAZ:00005218</oboInOwl:id>
        <oboInOwl:hasOBONamespace>GAZ</oboInOwl:hasOBONamespace>
        <rdfs:label>Department (Nicaragua)</rdfs:label>
    </rdf:Description>
    <rdf:Description rdf:about="http://purl.obolibrary.org/obo/GAZ_00005219">
        <rdfs:label>Chinandega Department</rdfs:label>
        <oboInOwl:id>GAZ:00005219</oboInOwl:id>
        <oboInOwl:hasOBONamespace>GAZ</oboInOwl:hasOBONamespace>
        <obo:IAO_0000115>A department in Nicaragua, located on the border with Honduras. The capital is the city of Chinandega.</obo:IAO_0000115>
    </rdf:Description>
    <rdf:Description rdf:about="http://purl.obolibrary.org/obo/GAZ_00005220">
        <rdfs:label>Chinandega</rdfs:label>
        <oboInOwl:hasOBONamespace>GAZ</oboInOwl:hasOBONamespace>
        <oboInOwl:id>GAZ:00005220</oboInOwl:id>
        <obo:IAO_0000115>A populated place. A town in Chinandega Department.</obo:IAO_0000115>
    </rdf:Description>
    <rdf:Description rdf:about="http://purl.obolibrary.org/obo/GAZ_00005221">
        <oboInOwl:hasOBONamespace>GAZ</oboInOwl:hasOBONamespace>
        <rdfs:label>populated place, Nicaragua</rdfs:label>
        <oboInOwl:id>GAZ:00005221</oboInOwl:id>
    </rdf:Description>
    <rdf:Description rdf:about="http://purl.obolibrary.org/obo/GAZ_00047242">
        <oboInOwl:hasOBONamespace>GAZ</oboInOwl:hasOBONamespace>
        <oboInOwl:id>GAZ:00047242</oboInOwl:id>
        <rdfs:label>Autonomous Region (Nicaragua)</rdfs:label>
    </rdf:Description>
    <rdf:Description rdf:about="http://purl.obolibrary.org/obo/GAZ_00047243">
        <rdfs:label>Region Autonoma del Atlantico Sur</rdfs:label>
        <oboInOwl:hasOBONamespace>GAZ</oboInOwl:hasOBONamespace>
        <oboInOwl:id>GAZ:00047243</oboInOwl:id>
        <obo:IAO_0000115>One of two autonomous regions in Nicaragua. The capital is Bluefields.</obo:IAO_0000115>
    </rdf:Description>
    <rdf:Description rdf:about="http://purl.obolibrary.org/obo/GAZ_00047244">
        <obo:IAO_0000115>One of two autonomous regions in Nicaragua. The capital is Puerto Cabezas.</obo:IAO_0000115>
        <rdfs:label>Region Autonoma del Atlantico Norte</rdfs:label>
        <oboInOwl:hasOBONamespace>GAZ</oboInOwl:hasOBONamespace>
        <oboInOwl:id>GAZ:00047244</oboInOwl:id>
    </rdf:Description>
    <rdf:Description rdf:about="http://purl.obolibrary.org/obo/GAZ_00047261">
        <obo:IAO_0000115>A department in Nicaragua. It was formed in 1957 from parts of Chontales and Zelaya. The capital is San Carlos. The Department also includes the Archipelago of Solentiname and the San Juan River, after which it is named.</obo:IAO_0000115>
        <oboInOwl:id>GAZ:00047261</oboInOwl:id>
        <oboInOwl:hasOBONamespace>GAZ</oboInOwl:hasOBONamespace>
        <rdfs:label>Rio San Juan Department</rdfs:label>
    </rdf:Description>
    <rdf:Description rdf:about="http://purl.obolibrary.org/obo/GAZ_00056193">
        <rdfs:label>Leon Department</rdfs:label>
        <oboInOwl:id>GAZ:00056193</oboInOwl:id>
        <oboInOwl:hasOBONamespace>GAZ</oboInOwl:hasOBONamespace>
        <obo:IAO_0000115>A department in Nicaragua. The capital is the city of Leon.</obo:IAO_0000115>
    </rdf:Description>
    <rdf:Description rdf:about="http://purl.obolibrary.org/obo/GAZ_00056201">
        <oboInOwl:hasOBONamespace>GAZ</oboInOwl:hasOBONamespace>
        <oboInOwl:id>GAZ:00056201</oboInOwl:id>
        <obo:IAO_0000115>A department in Nicaragua. The capital is the city of Masaya.</obo:IAO_0000115>
        <rdfs:label>Masaya Department</rdfs:label>
    </rdf:Description>
    <rdf:Description rdf:about="http://purl.obolibrary.org/obo/GAZ_00056204">
        <rdfs:label>Granada Department</rdfs:label>
        <oboInOwl:id>GAZ:00056204</oboInOwl:id>
        <obo:IAO_0000115>A department in Nicaragua. The capital is the city of Granada.</obo:IAO_0000115>
        <oboInOwl:hasOBONamespace>GAZ</oboInOwl:hasOBONamespace>
    </rdf:Description>
    <rdf:Description rdf:about="http://purl.obolibrary.org/obo/GAZ_00056208">
        <rdfs:label>Rivas Department</rdfs:label>
        <obo:IAO_0000115>A department of the Republic of Nicaragua. The department&apos;s capital is the city of Rivas.</obo:IAO_0000115>
        <oboInOwl:hasOBONamespace>GAZ</oboInOwl:hasOBONamespace>
        <oboInOwl:id>GAZ:00056208</oboInOwl:id>
    </rdf:Description>
    <rdf:Description rdf:about="http://purl.obolibrary.org/obo/GAZ_00056211">
        <oboInOwl:id>GAZ:00056211</oboInOwl:id>
        <oboInOwl:hasOBONamespace>GAZ</oboInOwl:hasOBONamespace>
        <obo:IAO_0000115>A department of Nicaragua. Its capital is the city of Esteli.</obo:IAO_0000115>
        <rdfs:label>Esteli Department</rdfs:label>
    </rdf:Description>
    <rdf:Description rdf:about="http://purl.obolibrary.org/obo/GAZ_00056214">
        <obo:IAO_0000115>A department in Nicaragua. It was formed in 1938 out of part of Chontales. The capital is the city of Boaco.</obo:IAO_0000115>
        <oboInOwl:id>GAZ:00056214</oboInOwl:id>
        <oboInOwl:hasOBONamespace>GAZ</oboInOwl:hasOBONamespace>
        <rdfs:label>Boaco Department</rdfs:label>
    </rdf:Description>
    <rdf:Description rdf:about="http://purl.obolibrary.org/obo/GAZ_00062427">
        <oboInOwl:hasOBONamespace>GAZ</oboInOwl:hasOBONamespace>
        <oboInOwl:id>GAZ:00062427</oboInOwl:id>
        <obo:IAO_0000115>A department in Nicaragua. It is bordered on the north by the country of Honduras. The departments surrounding it are, Matagalpa to the south, Zelaya to the east, and Esteli, Madriz, and Nueva Segovia.</obo:IAO_0000115>
        <rdfs:label>Jinotega Department</rdfs:label>
    </rdf:Description>
    <rdf:Description rdf:about="http://purl.obolibrary.org/obo/GAZ_00066798">
        <obo:IAO_0000115>A department in Nicaragua. The capital is Juigalpa.</obo:IAO_0000115>
        <rdfs:label>Chontales Department</rdfs:label>
        <oboInOwl:hasOBONamespace>GAZ</oboInOwl:hasOBONamespace>
        <oboInOwl:id>GAZ:00066798</oboInOwl:id>
    </rdf:Description>
    <rdf:Description rdf:about="http://purl.obolibrary.org/obo/GAZ_00066799">
        <obo:IAO_0000115>A department in Nicaragua. The capital is Jinotepe.</obo:IAO_0000115>
        <rdfs:label>Carazo Department</rdfs:label>
        <oboInOwl:id>GAZ:00066799</oboInOwl:id>
        <oboInOwl:hasOBONamespace>GAZ</oboInOwl:hasOBONamespace>
    </rdf:Description>
    <rdf:Description rdf:about="http://purl.obolibrary.org/obo/GAZ_00066800">
        <obo:IAO_0000115>A department in central Nicaragua. The capital is the city of Matagalpa.</obo:IAO_0000115>
        <oboInOwl:id>GAZ:00066800</oboInOwl:id>
        <oboInOwl:hasOBONamespace>GAZ</oboInOwl:hasOBONamespace>
        <rdfs:label>Matagalpa Department</rdfs:label>
    </rdf:Description>
    <rdf:Description rdf:about="http://purl.obolibrary.org/obo/GAZ_00066801">
        <obo:IAO_0000115>A department in Nicaragua. The capital is the city of Managua.</obo:IAO_0000115>
        <oboInOwl:hasOBONamespace>GAZ</oboInOwl:hasOBONamespace>
        <rdfs:label>Managua Department</rdfs:label>
        <oboInOwl:id>GAZ:00066801</oboInOwl:id>
    </rdf:Description>
    <rdf:Description rdf:about="http://purl.obolibrary.org/obo/GAZ_00066802">
        <oboInOwl:hasOBONamespace>GAZ</oboInOwl:hasOBONamespace>
        <rdfs:label>Nueva Segovia Department</rdfs:label>
        <obo:IAO_0000115>A department in Nicaragua. The capital is Ocotal.</obo:IAO_0000115>
        <oboInOwl:id>GAZ:00066802</oboInOwl:id>
    </rdf:Description>
    <rdf:Description rdf:about="http://purl.obolibrary.org/obo/GAZ_00066803">
        <rdfs:label>Madriz Department</rdfs:label>
        <oboInOwl:hasOBONamespace>GAZ</oboInOwl:hasOBONamespace>
        <oboInOwl:id>GAZ:00066803</oboInOwl:id>
        <obo:IAO_0000115>A department in Nicaragua. The capital is Somoto.</obo:IAO_0000115>
    </rdf:Description>
</rdf:RDF>



<!-- Generated by the OWL API (version 4.5.6) https://github.com/owlcs/owlapi -->

