<?xml version="1.0"?>
<rdf:RDF xmlns="http://purl.obolibrary.org/obo/gaz/subsets/countries/Niger.owl#"
     xml:base="http://purl.obolibrary.org/obo/gaz/subsets/countries/Niger.owl"
     xmlns:obo="http://purl.obolibrary.org/obo/"
     xmlns:owl="http://www.w3.org/2002/07/owl#"
     xmlns:rdf="http://www.w3.org/1999/02/22-rdf-syntax-ns#"
     xmlns:xml="http://www.w3.org/XML/1998/namespace"
     xmlns:xsd="http://www.w3.org/2001/XMLSchema#"
     xmlns:rdfs="http://www.w3.org/2000/01/rdf-schema#"
     xmlns:oboInOwl="http://www.geneontology.org/formats/oboInOwl#">
    <owl:Ontology rdf:about="http://purl.obolibrary.org/obo/gaz/subsets/countries/Niger.owl">
        <owl:imports rdf:resource="http://purl.obolibrary.org/obo/gaz/imports/envo_import.owl"/>
        <owl:imports rdf:resource="http://purl.obolibrary.org/obo/gaz/imports/ro_import.owl"/>
    </owl:Ontology>
    


    <!-- 
    ///////////////////////////////////////////////////////////////////////////////////////
    //
    // Annotation properties
    //
    ///////////////////////////////////////////////////////////////////////////////////////
     -->

    


    <!-- http://purl.obolibrary.org/obo/IAO_0000115 -->

    <owl:AnnotationProperty rdf:about="http://purl.obolibrary.org/obo/IAO_0000115"/>
    


    <!-- http://www.geneontology.org/formats/oboInOwl#hasOBONamespace -->

    <owl:AnnotationProperty rdf:about="http://www.geneontology.org/formats/oboInOwl#hasOBONamespace"/>
    


    <!-- http://www.geneontology.org/formats/oboInOwl#id -->

    <owl:AnnotationProperty rdf:about="http://www.geneontology.org/formats/oboInOwl#id"/>
    


    <!-- 
    ///////////////////////////////////////////////////////////////////////////////////////
    //
    // Object Properties
    //
    ///////////////////////////////////////////////////////////////////////////////////////
     -->

    


    <!-- http://purl.obolibrary.org/obo/RO_0001025 -->

    <owl:ObjectProperty rdf:about="http://purl.obolibrary.org/obo/RO_0001025"/>
    


    <!-- 
    ///////////////////////////////////////////////////////////////////////////////////////
    //
    // Classes
    //
    ///////////////////////////////////////////////////////////////////////////////////////
     -->

    


    <!-- http://purl.obolibrary.org/obo/ENVO_00000074 -->

    <owl:Class rdf:about="http://purl.obolibrary.org/obo/ENVO_00000074"/>
    


    <!-- http://purl.obolibrary.org/obo/ENVO_00000475 -->

    <owl:Class rdf:about="http://purl.obolibrary.org/obo/ENVO_00000475"/>
    


    <!-- http://purl.obolibrary.org/obo/GAZ_00000821 -->

    <owl:Class rdf:about="http://purl.obolibrary.org/obo/GAZ_00000821"/>
    


    <!-- http://purl.obolibrary.org/obo/GAZ_00000822 -->

    <owl:Class rdf:about="http://purl.obolibrary.org/obo/GAZ_00000822">
        <rdfs:subClassOf rdf:resource="http://purl.obolibrary.org/obo/GAZ_00000821"/>
    </owl:Class>
    


    <!-- http://purl.obolibrary.org/obo/GAZ_00000823 -->

    <owl:Class rdf:about="http://purl.obolibrary.org/obo/GAZ_00000823">
        <rdfs:subClassOf rdf:resource="http://purl.obolibrary.org/obo/GAZ_00000821"/>
    </owl:Class>
    


    <!-- http://purl.obolibrary.org/obo/GAZ_00000824 -->

    <owl:Class rdf:about="http://purl.obolibrary.org/obo/GAZ_00000824">
        <rdfs:subClassOf rdf:resource="http://purl.obolibrary.org/obo/GAZ_00000821"/>
    </owl:Class>
    


    <!-- http://purl.obolibrary.org/obo/GAZ_00000825 -->

    <owl:Class rdf:about="http://purl.obolibrary.org/obo/GAZ_00000825">
        <rdfs:subClassOf rdf:resource="http://purl.obolibrary.org/obo/GAZ_00000821"/>
    </owl:Class>
    


    <!-- http://purl.obolibrary.org/obo/GAZ_00000826 -->

    <owl:Class rdf:about="http://purl.obolibrary.org/obo/GAZ_00000826">
        <rdfs:subClassOf rdf:resource="http://purl.obolibrary.org/obo/GAZ_00000821"/>
    </owl:Class>
    


    <!-- http://purl.obolibrary.org/obo/GAZ_00000827 -->

    <owl:Class rdf:about="http://purl.obolibrary.org/obo/GAZ_00000827">
        <rdfs:subClassOf rdf:resource="http://purl.obolibrary.org/obo/GAZ_00000821"/>
    </owl:Class>
    


    <!-- http://purl.obolibrary.org/obo/GAZ_00000828 -->

    <owl:Class rdf:about="http://purl.obolibrary.org/obo/GAZ_00000828">
        <rdfs:subClassOf rdf:resource="http://purl.obolibrary.org/obo/GAZ_00000821"/>
    </owl:Class>
    


    <!-- http://purl.obolibrary.org/obo/GAZ_00000829 -->

    <owl:Class rdf:about="http://purl.obolibrary.org/obo/GAZ_00000829">
        <rdfs:subClassOf rdf:resource="http://purl.obolibrary.org/obo/GAZ_00001015"/>
    </owl:Class>
    


    <!-- http://purl.obolibrary.org/obo/GAZ_00001015 -->

    <owl:Class rdf:about="http://purl.obolibrary.org/obo/GAZ_00001015"/>
    


    <!-- http://purl.obolibrary.org/obo/GAZ_00058884 -->

    <owl:Class rdf:about="http://purl.obolibrary.org/obo/GAZ_00058884"/>
    


    <!-- http://purl.obolibrary.org/obo/GAZ_00058885 -->

    <owl:Class rdf:about="http://purl.obolibrary.org/obo/GAZ_00058885">
        <rdfs:subClassOf rdf:resource="http://purl.obolibrary.org/obo/GAZ_00058884"/>
        <obo:IAO_0000115>A cataract on the River Nile in Sudan near the confluence with the Atbara River.</obo:IAO_0000115>
        <oboInOwl:hasOBONamespace>GAZ</oboInOwl:hasOBONamespace>
        <oboInOwl:id>GAZ:00058885</oboInOwl:id>
        <rdfs:label>Fifth Cataract</rdfs:label>
    </owl:Class>
    


    <!-- http://purl.obolibrary.org/obo/GAZ_00058886 -->

    <owl:Class rdf:about="http://purl.obolibrary.org/obo/GAZ_00058886">
        <rdfs:subClassOf rdf:resource="http://purl.obolibrary.org/obo/GAZ_00058884"/>
    </owl:Class>
    


    <!-- http://purl.obolibrary.org/obo/GAZ_00058887 -->

    <owl:Class rdf:about="http://purl.obolibrary.org/obo/GAZ_00058887">
        <rdfs:subClassOf rdf:resource="http://purl.obolibrary.org/obo/GAZ_00058884"/>
        <obo:IAO_0000115>A former cataract on the River Nile in Sudan that was in Nubia and is now submerged in Lake Nasser.</obo:IAO_0000115>
        <oboInOwl:hasOBONamespace>GAZ</oboInOwl:hasOBONamespace>
        <oboInOwl:id>GAZ:00058887</oboInOwl:id>
        <rdfs:label>Second Cataract</rdfs:label>
    </owl:Class>
    


    <!-- http://purl.obolibrary.org/obo/GAZ_00058888 -->

    <owl:Class rdf:about="http://purl.obolibrary.org/obo/GAZ_00058888">
        <rdfs:subClassOf rdf:resource="http://purl.obolibrary.org/obo/GAZ_00058884"/>
        <obo:IAO_0000115>A cataract on the River Nile in Sudan near Tombos.</obo:IAO_0000115>
        <oboInOwl:hasOBONamespace>GAZ</oboInOwl:hasOBONamespace>
        <oboInOwl:id>GAZ:00058888</oboInOwl:id>
        <rdfs:label>Third Cataract</rdfs:label>
    </owl:Class>
    


    <!-- http://purl.obolibrary.org/obo/GAZ_00058889 -->

    <owl:Class rdf:about="http://purl.obolibrary.org/obo/GAZ_00058889">
        <rdfs:subClassOf rdf:resource="http://purl.obolibrary.org/obo/GAZ_00058884"/>
        <obo:IAO_0000115>A cataract on the River Nile in Sudan where it cuts through the Sabaluka pluton near Bagrawiyah.</obo:IAO_0000115>
        <oboInOwl:hasOBONamespace>GAZ</oboInOwl:hasOBONamespace>
        <oboInOwl:id>GAZ:00058889</oboInOwl:id>
        <rdfs:label>Sixth Cataract</rdfs:label>
    </owl:Class>
    


    <!-- http://purl.obolibrary.org/obo/GAZ_00058890 -->

    <owl:Class rdf:about="http://purl.obolibrary.org/obo/GAZ_00058890">
        <rdfs:subClassOf rdf:resource="http://purl.obolibrary.org/obo/GAZ_00058884"/>
    </owl:Class>
    


    <!-- http://purl.obolibrary.org/obo/GAZ_00230472 -->

    <owl:Class rdf:about="http://purl.obolibrary.org/obo/GAZ_00230472">
        <obo:IAO_0000115>A river. A tributary of the Qechene River.</obo:IAO_0000115>
        <oboInOwl:hasOBONamespace>GAZ</oboInOwl:hasOBONamespace>
        <oboInOwl:id>GAZ:00230472</oboInOwl:id>
        <rdfs:label>Ketama River</rdfs:label>
    </owl:Class>
    


    <!-- http://purl.obolibrary.org/obo/GAZ_00230473 -->

    <owl:Class rdf:about="http://purl.obolibrary.org/obo/GAZ_00230473">
        <obo:IAO_0000115>A river. A tributary of the Qechene River.</obo:IAO_0000115>
        <oboInOwl:hasOBONamespace>GAZ</oboInOwl:hasOBONamespace>
        <oboInOwl:id>GAZ:00230473</oboInOwl:id>
        <rdfs:label>Woia River</rdfs:label>
    </owl:Class>
    


    <!-- 
    ///////////////////////////////////////////////////////////////////////////////////////
    //
    // Individuals
    //
    ///////////////////////////////////////////////////////////////////////////////////////
     -->

    


    <!-- http://purl.obolibrary.org/obo/GAZ_00000585 -->

    <owl:NamedIndividual rdf:about="http://purl.obolibrary.org/obo/GAZ_00000585">
        <obo:IAO_0000115>A landlocked country in Western Africa, named after the Niger River. It borders Nigeria and Benin to the south, Burkina Faso and Mali to the west, Algeria and Libya to the north and Chad to the east. The capital city is Niamey. Niger is divided into 7 departments and one capital district. The departments are subdivided into 36 arrondissements and further subdivided into 129 communes.</obo:IAO_0000115>
        <oboInOwl:hasOBONamespace>GAZ</oboInOwl:hasOBONamespace>
        <oboInOwl:id>GAZ:00000585</oboInOwl:id>
        <rdfs:label>Niger</rdfs:label>
    </owl:NamedIndividual>
    


    <!-- http://purl.obolibrary.org/obo/GAZ_00000821 -->

    <owl:NamedIndividual rdf:about="http://purl.obolibrary.org/obo/GAZ_00000821">
        <obo:RO_0001025 rdf:resource="http://purl.obolibrary.org/obo/GAZ_00000585"/>
    </owl:NamedIndividual>
    


    <!-- http://purl.obolibrary.org/obo/GAZ_00000822 -->

    <owl:NamedIndividual rdf:about="http://purl.obolibrary.org/obo/GAZ_00000822"/>
    


    <!-- http://purl.obolibrary.org/obo/GAZ_00000823 -->

    <owl:NamedIndividual rdf:about="http://purl.obolibrary.org/obo/GAZ_00000823"/>
    


    <!-- http://purl.obolibrary.org/obo/GAZ_00000824 -->

    <owl:NamedIndividual rdf:about="http://purl.obolibrary.org/obo/GAZ_00000824"/>
    


    <!-- http://purl.obolibrary.org/obo/GAZ_00000825 -->

    <owl:NamedIndividual rdf:about="http://purl.obolibrary.org/obo/GAZ_00000825"/>
    


    <!-- http://purl.obolibrary.org/obo/GAZ_00000826 -->

    <owl:NamedIndividual rdf:about="http://purl.obolibrary.org/obo/GAZ_00000826"/>
    


    <!-- http://purl.obolibrary.org/obo/GAZ_00000827 -->

    <owl:NamedIndividual rdf:about="http://purl.obolibrary.org/obo/GAZ_00000827"/>
    


    <!-- http://purl.obolibrary.org/obo/GAZ_00000828 -->

    <owl:NamedIndividual rdf:about="http://purl.obolibrary.org/obo/GAZ_00000828"/>
    


    <!-- http://purl.obolibrary.org/obo/GAZ_00000829 -->

    <owl:NamedIndividual rdf:about="http://purl.obolibrary.org/obo/GAZ_00000829"/>
    


    <!-- http://purl.obolibrary.org/obo/GAZ_00001015 -->

    <owl:NamedIndividual rdf:about="http://purl.obolibrary.org/obo/GAZ_00001015">
        <obo:RO_0001025 rdf:resource="http://purl.obolibrary.org/obo/GAZ_00000585"/>
    </owl:NamedIndividual>
    


    <!-- http://purl.obolibrary.org/obo/GAZ_00004033 -->

    <owl:NamedIndividual rdf:about="http://purl.obolibrary.org/obo/GAZ_00004033">
        <oboInOwl:hasOBONamespace>GAZ</oboInOwl:hasOBONamespace>
        <oboInOwl:id>GAZ:00004033</oboInOwl:id>
        <rdfs:label>Northern Sahara Desert</rdfs:label>
    </owl:NamedIndividual>
    


    <!-- http://purl.obolibrary.org/obo/GAZ_00009949 -->

    <owl:NamedIndividual rdf:about="http://purl.obolibrary.org/obo/GAZ_00009949">
        <obo:IAO_0000115>The delta formed in Northern Egypt where the Nile River spreads out and drains into the Mediterranean Sea. It is one of the world&apos;s largest river delta, from Alexandria in the west to Port Said in the east, it covers some 240 km of Mediterranean coastline.</obo:IAO_0000115>
        <oboInOwl:hasOBONamespace>GAZ</oboInOwl:hasOBONamespace>
        <oboInOwl:id>GAZ:00009949</oboInOwl:id>
        <rdfs:label>Nile Delta</rdfs:label>
    </owl:NamedIndividual>
    


    <!-- http://purl.obolibrary.org/obo/GAZ_00031012 -->

    <owl:NamedIndividual rdf:about="http://purl.obolibrary.org/obo/GAZ_00031012">
        <obo:RO_0001025 rdf:resource="http://purl.obolibrary.org/obo/GAZ_00051197"/>
        <obo:IAO_0000115>One of the seven oases of the Western Desert of Egypt (part of the Libyan Desert). Dakhla Oasis is located at 350 km from the Nile Valley and is also situated between the oases of Farafra and Kharga. It measures some 80 km from east to west and about 25 km from north to south.</obo:IAO_0000115>
        <oboInOwl:hasOBONamespace>GAZ</oboInOwl:hasOBONamespace>
        <oboInOwl:id>GAZ:00031012</oboInOwl:id>
        <rdfs:label>Dakhla Oasis</rdfs:label>
    </owl:NamedIndividual>
    


    <!-- http://purl.obolibrary.org/obo/GAZ_00031013 -->

    <owl:NamedIndividual rdf:about="http://purl.obolibrary.org/obo/GAZ_00031013">
        <obo:RO_0001025 rdf:resource="http://purl.obolibrary.org/obo/GAZ_00051197"/>
        <obo:IAO_0000115>The southernmost of Egypt&apos;s five western oases. It is located in the Libyan Desert, about 200 km to the west of the Nile valley, and is some 150 km long. It is located in and is the capital of El Wadi el Gedid governorate.</obo:IAO_0000115>
        <oboInOwl:hasOBONamespace>GAZ</oboInOwl:hasOBONamespace>
        <oboInOwl:id>GAZ:00031013</oboInOwl:id>
        <rdfs:label>Kharga Oasis</rdfs:label>
    </owl:NamedIndividual>
    


    <!-- http://purl.obolibrary.org/obo/GAZ_00031014 -->

    <owl:NamedIndividual rdf:about="http://purl.obolibrary.org/obo/GAZ_00031014">
        <obo:RO_0001025 rdf:resource="http://purl.obolibrary.org/obo/GAZ_00051197"/>
        <oboInOwl:hasOBONamespace>GAZ</oboInOwl:hasOBONamespace>
        <oboInOwl:id>GAZ:00031014</oboInOwl:id>
        <rdfs:label>Baris Oasis</rdfs:label>
    </owl:NamedIndividual>
    


    <!-- http://purl.obolibrary.org/obo/GAZ_00031015 -->

    <owl:NamedIndividual rdf:about="http://purl.obolibrary.org/obo/GAZ_00031015">
        <obo:RO_0001025 rdf:resource="http://purl.obolibrary.org/obo/GAZ_00051197"/>
        <obo:IAO_0000115>The smallest oasis located in Western Egypt. It is located in the Libyan Desert, approximately mid-way between Dakhla and Bahariya.</obo:IAO_0000115>
        <oboInOwl:hasOBONamespace>GAZ</oboInOwl:hasOBONamespace>
        <oboInOwl:id>GAZ:00031015</oboInOwl:id>
        <rdfs:label>Farafra Oasis</rdfs:label>
    </owl:NamedIndividual>
    


    <!-- http://purl.obolibrary.org/obo/GAZ_00032115 -->

    <owl:NamedIndividual rdf:about="http://purl.obolibrary.org/obo/GAZ_00032115">
        <obo:RO_0001025 rdf:resource="http://purl.obolibrary.org/obo/GAZ_00000822"/>
        <obo:IAO_0000115>A department of the Agadez Region in Niger. Its capital lies at the city of Bilma.</obo:IAO_0000115>
        <oboInOwl:hasOBONamespace>GAZ</oboInOwl:hasOBONamespace>
        <oboInOwl:id>GAZ:00032115</oboInOwl:id>
        <rdfs:label>Bilma Department</rdfs:label>
    </owl:NamedIndividual>
    


    <!-- http://purl.obolibrary.org/obo/GAZ_00032116 -->

    <owl:NamedIndividual rdf:about="http://purl.obolibrary.org/obo/GAZ_00032116">
        <obo:RO_0001025 rdf:resource="http://purl.obolibrary.org/obo/GAZ_00000822"/>
        <obo:IAO_0000115>A department of the Agadez Region in Niger. Its capital lies at the city of Tchirozerine.</obo:IAO_0000115>
        <oboInOwl:hasOBONamespace>GAZ</oboInOwl:hasOBONamespace>
        <oboInOwl:id>GAZ:00032116</oboInOwl:id>
        <rdfs:label>Tchirozerine Department</rdfs:label>
    </owl:NamedIndividual>
    


    <!-- http://purl.obolibrary.org/obo/GAZ_00032117 -->

    <owl:NamedIndividual rdf:about="http://purl.obolibrary.org/obo/GAZ_00032117">
        <obo:RO_0001025 rdf:resource="http://purl.obolibrary.org/obo/GAZ_00000823"/>
        <obo:IAO_0000115>A department of the Diffa Region in Niger. Its capital lies at the city of Maine-soroa.</obo:IAO_0000115>
        <oboInOwl:hasOBONamespace>GAZ</oboInOwl:hasOBONamespace>
        <oboInOwl:id>GAZ:00032117</oboInOwl:id>
        <rdfs:label>Maine-soroa Department</rdfs:label>
    </owl:NamedIndividual>
    


    <!-- http://purl.obolibrary.org/obo/GAZ_00032118 -->

    <owl:NamedIndividual rdf:about="http://purl.obolibrary.org/obo/GAZ_00032118">
        <obo:RO_0001025 rdf:resource="http://purl.obolibrary.org/obo/GAZ_00000823"/>
        <obo:IAO_0000115>A department of the Diffa Region in Niger. Its capital lies at the city of Diffa.</obo:IAO_0000115>
        <oboInOwl:hasOBONamespace>GAZ</oboInOwl:hasOBONamespace>
        <oboInOwl:id>GAZ:00032118</oboInOwl:id>
        <rdfs:label>Diffa Department</rdfs:label>
    </owl:NamedIndividual>
    


    <!-- http://purl.obolibrary.org/obo/GAZ_00032119 -->

    <owl:NamedIndividual rdf:about="http://purl.obolibrary.org/obo/GAZ_00032119">
        <obo:RO_0001025 rdf:resource="http://purl.obolibrary.org/obo/GAZ_00000823"/>
        <obo:IAO_0000115>A department of the Diffa Region in Niger. Its capital lies at the city of N&apos;guigmi.</obo:IAO_0000115>
        <oboInOwl:hasOBONamespace>GAZ</oboInOwl:hasOBONamespace>
        <oboInOwl:id>GAZ:00032119</oboInOwl:id>
        <rdfs:label>N&apos;guigmi Department</rdfs:label>
    </owl:NamedIndividual>
    


    <!-- http://purl.obolibrary.org/obo/GAZ_00032120 -->

    <owl:NamedIndividual rdf:about="http://purl.obolibrary.org/obo/GAZ_00032120">
        <obo:RO_0001025 rdf:resource="http://purl.obolibrary.org/obo/GAZ_00000824"/>
        <obo:IAO_0000115>A department of the Dosso Region in Niger. Its capital lies at the city of Dosso.</obo:IAO_0000115>
        <oboInOwl:hasOBONamespace>GAZ</oboInOwl:hasOBONamespace>
        <oboInOwl:id>GAZ:00032120</oboInOwl:id>
        <rdfs:label>Dosso Department</rdfs:label>
    </owl:NamedIndividual>
    


    <!-- http://purl.obolibrary.org/obo/GAZ_00032121 -->

    <owl:NamedIndividual rdf:about="http://purl.obolibrary.org/obo/GAZ_00032121">
        <obo:RO_0001025 rdf:resource="http://purl.obolibrary.org/obo/GAZ_00000824"/>
        <obo:IAO_0000115>A department of the Dosso Region in Niger. Its capital lies at the city of Loga.</obo:IAO_0000115>
        <oboInOwl:hasOBONamespace>GAZ</oboInOwl:hasOBONamespace>
        <oboInOwl:id>GAZ:00032121</oboInOwl:id>
        <rdfs:label>Loga Department</rdfs:label>
    </owl:NamedIndividual>
    


    <!-- http://purl.obolibrary.org/obo/GAZ_00032122 -->

    <owl:NamedIndividual rdf:about="http://purl.obolibrary.org/obo/GAZ_00032122">
        <obo:RO_0001025 rdf:resource="http://purl.obolibrary.org/obo/GAZ_00000824"/>
        <obo:IAO_0000115>A department of the Dosso Region in Niger. Its capital lies at the city of Boboye.</obo:IAO_0000115>
        <oboInOwl:hasOBONamespace>GAZ</oboInOwl:hasOBONamespace>
        <oboInOwl:id>GAZ:00032122</oboInOwl:id>
        <rdfs:label>Boboye Department</rdfs:label>
    </owl:NamedIndividual>
    


    <!-- http://purl.obolibrary.org/obo/GAZ_00032123 -->

    <owl:NamedIndividual rdf:about="http://purl.obolibrary.org/obo/GAZ_00032123">
        <obo:RO_0001025 rdf:resource="http://purl.obolibrary.org/obo/GAZ_00000824"/>
        <obo:IAO_0000115>A department of the Dosso Region in Niger. Its capital lies at the city of Gaya.</obo:IAO_0000115>
        <oboInOwl:hasOBONamespace>GAZ</oboInOwl:hasOBONamespace>
        <oboInOwl:id>GAZ:00032123</oboInOwl:id>
        <rdfs:label>Gaya Department</rdfs:label>
    </owl:NamedIndividual>
    


    <!-- http://purl.obolibrary.org/obo/GAZ_00032124 -->

    <owl:NamedIndividual rdf:about="http://purl.obolibrary.org/obo/GAZ_00032124">
        <obo:RO_0001025 rdf:resource="http://purl.obolibrary.org/obo/GAZ_00000824"/>
        <obo:IAO_0000115>A department of the Dosso Region in Niger. Its capital lies at the city of Dogondoutchi.</obo:IAO_0000115>
        <oboInOwl:hasOBONamespace>GAZ</oboInOwl:hasOBONamespace>
        <oboInOwl:id>GAZ:00032124</oboInOwl:id>
        <rdfs:label>Dogondoutchi Department</rdfs:label>
    </owl:NamedIndividual>
    


    <!-- http://purl.obolibrary.org/obo/GAZ_00032125 -->

    <owl:NamedIndividual rdf:about="http://purl.obolibrary.org/obo/GAZ_00032125">
        <obo:RO_0001025 rdf:resource="http://purl.obolibrary.org/obo/GAZ_00000825"/>
        <obo:IAO_0000115>A department of the Maradi Region in Niger. Its capital lies at the city of Mayahi.</obo:IAO_0000115>
        <oboInOwl:hasOBONamespace>GAZ</oboInOwl:hasOBONamespace>
        <oboInOwl:id>GAZ:00032125</oboInOwl:id>
        <rdfs:label>Mayahi Department</rdfs:label>
    </owl:NamedIndividual>
    


    <!-- http://purl.obolibrary.org/obo/GAZ_00032126 -->

    <owl:NamedIndividual rdf:about="http://purl.obolibrary.org/obo/GAZ_00032126">
        <obo:RO_0001025 rdf:resource="http://purl.obolibrary.org/obo/GAZ_00000825"/>
        <obo:IAO_0000115>A department of the Maradi Region in Niger. Its capital lies at the city of Tessaoua.</obo:IAO_0000115>
        <oboInOwl:hasOBONamespace>GAZ</oboInOwl:hasOBONamespace>
        <oboInOwl:id>GAZ:00032126</oboInOwl:id>
        <rdfs:label>Tessaoua Department</rdfs:label>
    </owl:NamedIndividual>
    


    <!-- http://purl.obolibrary.org/obo/GAZ_00032127 -->

    <owl:NamedIndividual rdf:about="http://purl.obolibrary.org/obo/GAZ_00032127">
        <obo:RO_0001025 rdf:resource="http://purl.obolibrary.org/obo/GAZ_00000825"/>
        <obo:IAO_0000115>A department of the Maradi Region in Niger. Its capital lies at the city of Aguie.</obo:IAO_0000115>
        <oboInOwl:hasOBONamespace>GAZ</oboInOwl:hasOBONamespace>
        <oboInOwl:id>GAZ:00032127</oboInOwl:id>
        <rdfs:label>Aguie Department</rdfs:label>
    </owl:NamedIndividual>
    


    <!-- http://purl.obolibrary.org/obo/GAZ_00032128 -->

    <owl:NamedIndividual rdf:about="http://purl.obolibrary.org/obo/GAZ_00032128">
        <obo:RO_0001025 rdf:resource="http://purl.obolibrary.org/obo/GAZ_00000825"/>
        <obo:IAO_0000115>A department of the Maradi Region in Niger. Its capital lies at the city of Groumdji.</obo:IAO_0000115>
        <oboInOwl:hasOBONamespace>GAZ</oboInOwl:hasOBONamespace>
        <oboInOwl:id>GAZ:00032128</oboInOwl:id>
        <rdfs:label>Groumdji Department</rdfs:label>
    </owl:NamedIndividual>
    


    <!-- http://purl.obolibrary.org/obo/GAZ_00032129 -->

    <owl:NamedIndividual rdf:about="http://purl.obolibrary.org/obo/GAZ_00032129">
        <obo:RO_0001025 rdf:resource="http://purl.obolibrary.org/obo/GAZ_00000825"/>
        <obo:IAO_0000115>A department of the Maradi Region in Niger. Its capital lies at the city of Madarounfa.</obo:IAO_0000115>
        <oboInOwl:hasOBONamespace>GAZ</oboInOwl:hasOBONamespace>
        <oboInOwl:id>GAZ:00032129</oboInOwl:id>
        <rdfs:label>Madarounfa Department</rdfs:label>
    </owl:NamedIndividual>
    


    <!-- http://purl.obolibrary.org/obo/GAZ_00032130 -->

    <owl:NamedIndividual rdf:about="http://purl.obolibrary.org/obo/GAZ_00032130">
        <obo:RO_0001025 rdf:resource="http://purl.obolibrary.org/obo/GAZ_00000825"/>
        <obo:IAO_0000115>A department of the Maradi Region in Niger. Its capital lies at the city of Dakoro.</obo:IAO_0000115>
        <oboInOwl:hasOBONamespace>GAZ</oboInOwl:hasOBONamespace>
        <oboInOwl:id>GAZ:00032130</oboInOwl:id>
        <rdfs:label>Dakoro Department</rdfs:label>
    </owl:NamedIndividual>
    


    <!-- http://purl.obolibrary.org/obo/GAZ_00032132 -->

    <owl:NamedIndividual rdf:about="http://purl.obolibrary.org/obo/GAZ_00032132">
        <obo:RO_0001025 rdf:resource="http://purl.obolibrary.org/obo/GAZ_00000826"/>
        <obo:IAO_0000115>A department of the Tahoua Region in Niger. Its capital lies at the city of Bouza, and also includes the town of Deoule.</obo:IAO_0000115>
        <oboInOwl:hasOBONamespace>GAZ</oboInOwl:hasOBONamespace>
        <oboInOwl:id>GAZ:00032132</oboInOwl:id>
        <rdfs:label>Bouza Department</rdfs:label>
    </owl:NamedIndividual>
    


    <!-- http://purl.obolibrary.org/obo/GAZ_00032133 -->

    <owl:NamedIndividual rdf:about="http://purl.obolibrary.org/obo/GAZ_00032133">
        <obo:RO_0001025 rdf:resource="http://purl.obolibrary.org/obo/GAZ_00000826"/>
        <obo:IAO_0000115>A department of the Tahoua Region in Niger. Its capital lies at the city of Keita.</obo:IAO_0000115>
        <oboInOwl:hasOBONamespace>GAZ</oboInOwl:hasOBONamespace>
        <oboInOwl:id>GAZ:00032133</oboInOwl:id>
        <rdfs:label>Keita Department</rdfs:label>
    </owl:NamedIndividual>
    


    <!-- http://purl.obolibrary.org/obo/GAZ_00032134 -->

    <owl:NamedIndividual rdf:about="http://purl.obolibrary.org/obo/GAZ_00032134">
        <obo:RO_0001025 rdf:resource="http://purl.obolibrary.org/obo/GAZ_00000826"/>
        <obo:IAO_0000115>A department of the Tahoua Region in Niger. Its capital lies at the city of Illela.</obo:IAO_0000115>
        <oboInOwl:hasOBONamespace>GAZ</oboInOwl:hasOBONamespace>
        <oboInOwl:id>GAZ:00032134</oboInOwl:id>
        <rdfs:label>Illela Department</rdfs:label>
    </owl:NamedIndividual>
    


    <!-- http://purl.obolibrary.org/obo/GAZ_00032135 -->

    <owl:NamedIndividual rdf:about="http://purl.obolibrary.org/obo/GAZ_00032135">
        <obo:RO_0001025 rdf:resource="http://purl.obolibrary.org/obo/GAZ_00000826"/>
        <obo:IAO_0000115>A department of the Tahoua Region in Niger. Its capital lies at the city of Madoua.</obo:IAO_0000115>
        <oboInOwl:hasOBONamespace>GAZ</oboInOwl:hasOBONamespace>
        <oboInOwl:id>GAZ:00032135</oboInOwl:id>
        <rdfs:label>Madoua Department</rdfs:label>
    </owl:NamedIndividual>
    


    <!-- http://purl.obolibrary.org/obo/GAZ_00032137 -->

    <owl:NamedIndividual rdf:about="http://purl.obolibrary.org/obo/GAZ_00032137">
        <obo:RO_0001025 rdf:resource="http://purl.obolibrary.org/obo/GAZ_00000826"/>
        <obo:IAO_0000115>A department of the Tahoua Region in Niger. Its capital lies at the city of Tahoua It includes the towns of Bambay and Kalkou.</obo:IAO_0000115>
        <oboInOwl:hasOBONamespace>GAZ</oboInOwl:hasOBONamespace>
        <oboInOwl:id>GAZ:00032137</oboInOwl:id>
        <rdfs:label>Tahoua Department</rdfs:label>
    </owl:NamedIndividual>
    


    <!-- http://purl.obolibrary.org/obo/GAZ_00032138 -->

    <owl:NamedIndividual rdf:about="http://purl.obolibrary.org/obo/GAZ_00032138">
        <obo:RO_0001025 rdf:resource="http://purl.obolibrary.org/obo/GAZ_00000826"/>
        <obo:IAO_0000115>A department of the Tahoua Region in Niger. Its capital lies at the city of Tchin-Tabaraden.</obo:IAO_0000115>
        <oboInOwl:hasOBONamespace>GAZ</oboInOwl:hasOBONamespace>
        <oboInOwl:id>GAZ:00032138</oboInOwl:id>
        <rdfs:label>Tchin-Tabaraden Department</rdfs:label>
    </owl:NamedIndividual>
    


    <!-- http://purl.obolibrary.org/obo/GAZ_00032139 -->

    <owl:NamedIndividual rdf:about="http://purl.obolibrary.org/obo/GAZ_00032139">
        <obo:RO_0001025 rdf:resource="http://purl.obolibrary.org/obo/GAZ_00000827"/>
        <obo:IAO_0000115>A department of the Tillaberi Region in Niger. Its capital lies at the city of Oullam, which is designated an Urban Commune. The department also includes the Rural Communes of Simiri and Tondikiwindi, as well as the towns of Bani Bangou and Dingazi.</obo:IAO_0000115>
        <oboInOwl:hasOBONamespace>GAZ</oboInOwl:hasOBONamespace>
        <oboInOwl:id>GAZ:00032139</oboInOwl:id>
        <rdfs:label>Ouallam Department</rdfs:label>
    </owl:NamedIndividual>
    


    <!-- http://purl.obolibrary.org/obo/GAZ_00032140 -->

    <owl:NamedIndividual rdf:about="http://purl.obolibrary.org/obo/GAZ_00032140">
        <obo:RO_0001025 rdf:resource="http://purl.obolibrary.org/obo/GAZ_00000827"/>
        <obo:IAO_0000115>A department of the Tillaberi Region in Niger. Its capital lies at the city of Tillaberi, and contains the Communes of Ayorou, Anzourou, Dessa, Kourteye, and Sinder. Tillaberi is also the capital of Tillaberi Region. The western border of the Department is formed by the Niger River.</obo:IAO_0000115>
        <oboInOwl:hasOBONamespace>GAZ</oboInOwl:hasOBONamespace>
        <oboInOwl:id>GAZ:00032140</oboInOwl:id>
        <rdfs:label>Tillaberi Department</rdfs:label>
    </owl:NamedIndividual>
    


    <!-- http://purl.obolibrary.org/obo/GAZ_00032141 -->

    <owl:NamedIndividual rdf:about="http://purl.obolibrary.org/obo/GAZ_00032141">
        <obo:RO_0001025 rdf:resource="http://purl.obolibrary.org/obo/GAZ_00000827"/>
        <obo:IAO_0000115>A department of the Tillaberi Region in Niger. Its capital lies at the city of Kollo, and includes the towns of N&apos;Dounga, Fakara, Hamdallay, Karma, Kirtachi, Koure, Lamorde, Libore, and Namaro.</obo:IAO_0000115>
        <oboInOwl:hasOBONamespace>GAZ</oboInOwl:hasOBONamespace>
        <oboInOwl:id>GAZ:00032141</oboInOwl:id>
        <rdfs:label>Kollo Department</rdfs:label>
    </owl:NamedIndividual>
    


    <!-- http://purl.obolibrary.org/obo/GAZ_00032142 -->

    <owl:NamedIndividual rdf:about="http://purl.obolibrary.org/obo/GAZ_00032142">
        <obo:RO_0001025 rdf:resource="http://purl.obolibrary.org/obo/GAZ_00000827"/>
        <obo:IAO_0000115>A department of the Tillaberi Region in Niger. Its capital city is Say, and includes the towns of Gueladjo, Tamou, and Torodi.</obo:IAO_0000115>
        <oboInOwl:hasOBONamespace>GAZ</oboInOwl:hasOBONamespace>
        <oboInOwl:id>GAZ:00032142</oboInOwl:id>
        <rdfs:label>Say Department</rdfs:label>
    </owl:NamedIndividual>
    


    <!-- http://purl.obolibrary.org/obo/GAZ_00032143 -->

    <owl:NamedIndividual rdf:about="http://purl.obolibrary.org/obo/GAZ_00032143">
        <obo:RO_0001025 rdf:resource="http://purl.obolibrary.org/obo/GAZ_00000827"/>
        <obo:IAO_0000115>A department of the Tillaberi Region in Niger. Its capital lies at the city of Tera.</obo:IAO_0000115>
        <oboInOwl:hasOBONamespace>GAZ</oboInOwl:hasOBONamespace>
        <oboInOwl:id>GAZ:00032143</oboInOwl:id>
        <rdfs:label>Tera Department</rdfs:label>
    </owl:NamedIndividual>
    


    <!-- http://purl.obolibrary.org/obo/GAZ_00032144 -->

    <owl:NamedIndividual rdf:about="http://purl.obolibrary.org/obo/GAZ_00032144">
        <obo:RO_0001025 rdf:resource="http://purl.obolibrary.org/obo/GAZ_00000827"/>
        <obo:IAO_0000115>A department of the Tillaberi Region in Niger. Its capital lies at the city of Filingue, and includes the towns of Konfey, Bonkoukou, Tabala, and Tondikandia.</obo:IAO_0000115>
        <oboInOwl:hasOBONamespace>GAZ</oboInOwl:hasOBONamespace>
        <oboInOwl:id>GAZ:00032144</oboInOwl:id>
        <rdfs:label>Filingue Department</rdfs:label>
    </owl:NamedIndividual>
    


    <!-- http://purl.obolibrary.org/obo/GAZ_00032145 -->

    <owl:NamedIndividual rdf:about="http://purl.obolibrary.org/obo/GAZ_00032145">
        <obo:RO_0001025 rdf:resource="http://purl.obolibrary.org/obo/GAZ_00000828"/>
        <obo:IAO_0000115>A department of the Zinder Region in Niger. Its capital lies at the city of Goure.</obo:IAO_0000115>
        <oboInOwl:hasOBONamespace>GAZ</oboInOwl:hasOBONamespace>
        <oboInOwl:id>GAZ:00032145</oboInOwl:id>
        <rdfs:label>Goure Department</rdfs:label>
    </owl:NamedIndividual>
    


    <!-- http://purl.obolibrary.org/obo/GAZ_00032146 -->

    <owl:NamedIndividual rdf:about="http://purl.obolibrary.org/obo/GAZ_00032146">
        <obo:RO_0001025 rdf:resource="http://purl.obolibrary.org/obo/GAZ_00000828"/>
        <obo:IAO_0000115>A department of the Zinder Region in Niger. Its capital lies at the city of Matameye.</obo:IAO_0000115>
        <oboInOwl:hasOBONamespace>GAZ</oboInOwl:hasOBONamespace>
        <oboInOwl:id>GAZ:00032146</oboInOwl:id>
        <rdfs:label>Matameye Department</rdfs:label>
    </owl:NamedIndividual>
    


    <!-- http://purl.obolibrary.org/obo/GAZ_00032147 -->

    <owl:NamedIndividual rdf:about="http://purl.obolibrary.org/obo/GAZ_00032147">
        <obo:RO_0001025 rdf:resource="http://purl.obolibrary.org/obo/GAZ_00000828"/>
        <obo:IAO_0000115>A department of the Zinder Region in Niger. Its capital lies at the city of Tanout.</obo:IAO_0000115>
        <oboInOwl:hasOBONamespace>GAZ</oboInOwl:hasOBONamespace>
        <oboInOwl:id>GAZ:00032147</oboInOwl:id>
        <rdfs:label>Tanout Department</rdfs:label>
    </owl:NamedIndividual>
    


    <!-- http://purl.obolibrary.org/obo/GAZ_00032148 -->

    <owl:NamedIndividual rdf:about="http://purl.obolibrary.org/obo/GAZ_00032148">
        <obo:RO_0001025 rdf:resource="http://purl.obolibrary.org/obo/GAZ_00000828"/>
        <obo:IAO_0000115>A department of the Zinder Region in Niger. Its capital lies at the city of Mirriah.</obo:IAO_0000115>
        <oboInOwl:hasOBONamespace>GAZ</oboInOwl:hasOBONamespace>
        <oboInOwl:id>GAZ:00032148</oboInOwl:id>
        <rdfs:label>Mirriah Department</rdfs:label>
    </owl:NamedIndividual>
    


    <!-- http://purl.obolibrary.org/obo/GAZ_00032149 -->

    <owl:NamedIndividual rdf:about="http://purl.obolibrary.org/obo/GAZ_00032149">
        <obo:RO_0001025 rdf:resource="http://purl.obolibrary.org/obo/GAZ_00000828"/>
        <obo:IAO_0000115>A department of the Zinder Region in Niger. Its capital lies at the city of Magaria.</obo:IAO_0000115>
        <oboInOwl:hasOBONamespace>GAZ</oboInOwl:hasOBONamespace>
        <oboInOwl:id>GAZ:00032149</oboInOwl:id>
        <rdfs:label>Magaria Department</rdfs:label>
    </owl:NamedIndividual>
    


    <!-- http://purl.obolibrary.org/obo/GAZ_00043227 -->

    <owl:NamedIndividual rdf:about="http://purl.obolibrary.org/obo/GAZ_00043227">
        <obo:IAO_0000115>An island located just to the south of Aswan.</obo:IAO_0000115>
        <oboInOwl:hasOBONamespace>GAZ</oboInOwl:hasOBONamespace>
        <oboInOwl:id>GAZ:00043227</oboInOwl:id>
        <rdfs:label>Sehel Island</rdfs:label>
    </owl:NamedIndividual>
    


    <!-- http://purl.obolibrary.org/obo/GAZ_00044902 -->

    <owl:NamedIndividual rdf:about="http://purl.obolibrary.org/obo/GAZ_00044902">
        <obo:IAO_0000115>A reservoir in Egypt and northern Sudan created as a result of the construction of the Aswan High Dam across the waters of the Nile between 1958 and 1970. The lake is some 550 km long and 35 km across at its widest point, which is near the Tropic of Cancer. It covers a total surface area of 5,250 km2 and has a storage capacity of some 157 km2 of water.</obo:IAO_0000115>
        <oboInOwl:hasOBONamespace>GAZ</oboInOwl:hasOBONamespace>
        <oboInOwl:id>GAZ:00044902</oboInOwl:id>
        <rdfs:label>Lake Nasser</rdfs:label>
    </owl:NamedIndividual>
    


    <!-- http://purl.obolibrary.org/obo/GAZ_00051196 -->

    <owl:NamedIndividual rdf:about="http://purl.obolibrary.org/obo/GAZ_00051196">
        <obo:RO_0001025 rdf:resource="http://purl.obolibrary.org/obo/GAZ_00051197"/>
        <obo:IAO_0000115>A desert basin within the Libyan Desert of north-western Egypt. It is bounded by a steep, and in places precipitous, escarpment, along the northwestern and northern sides, which rises to heights of over 300 m, and a few km away from the escarpment edge, to over 500 m. By contrast the southern and eastern sides of the depression rise more gradually to the plateau of the Western Desert. Saline marshes/deserts, up to 30 km wide and over 150 km long, are situated under the escarpment along the northern side of the depression, and other marshes extend out into the southern central part of the basin.</obo:IAO_0000115>
        <oboInOwl:hasOBONamespace>GAZ</oboInOwl:hasOBONamespace>
        <oboInOwl:id>GAZ:00051196</oboInOwl:id>
        <rdfs:label>Qattara Depression</rdfs:label>
    </owl:NamedIndividual>
    


    <!-- http://purl.obolibrary.org/obo/GAZ_00051197 -->

    <owl:NamedIndividual rdf:about="http://purl.obolibrary.org/obo/GAZ_00051197">
        <obo:IAO_0000115>A desert that is located in the northern and eastern part of the Sahara Desert and occupies southwestern Egypt, eastern Libya and northwestern Sudan. Covering an area of approximately 1,100,000 km2 it extends approximately 1,100 km from east to west, and 1,000 km from north to south, in about the shape of a rectangle.</obo:IAO_0000115>
        <oboInOwl:hasOBONamespace>GAZ</oboInOwl:hasOBONamespace>
        <oboInOwl:id>GAZ:00051197</oboInOwl:id>
        <rdfs:label>Libyan Desert</rdfs:label>
    </owl:NamedIndividual>
    


    <!-- http://purl.obolibrary.org/obo/GAZ_00051198 -->

    <owl:NamedIndividual rdf:about="http://purl.obolibrary.org/obo/GAZ_00051198">
        <obo:IAO_0000115>A desert region in the south central Sahara. It comprises a vast plain of sand stretching from northeastern Niger into western Chad, occupying an area of over 400,000 km2). Its boundaries are conventionally said to be the Air Mountains in the west, the Ahaggar Mountains in the north, the Djado Plateau in the northeast, the Tibesti Mountains in the east and the basin of Lake Chad in the south.</obo:IAO_0000115>
        <oboInOwl:hasOBONamespace>GAZ</oboInOwl:hasOBONamespace>
        <oboInOwl:id>GAZ:00051198</oboInOwl:id>
        <rdfs:label>Erg of Tenere</rdfs:label>
    </owl:NamedIndividual>
    


    <!-- http://purl.obolibrary.org/obo/GAZ_00051199 -->

    <owl:NamedIndividual rdf:about="http://purl.obolibrary.org/obo/GAZ_00051199">
        <obo:RO_0001025 rdf:resource="http://purl.obolibrary.org/obo/GAZ_00051197"/>
        <obo:IAO_0000115>A sand sea.</obo:IAO_0000115>
        <oboInOwl:hasOBONamespace>GAZ</oboInOwl:hasOBONamespace>
        <oboInOwl:id>GAZ:00051199</oboInOwl:id>
        <rdfs:label>Rebiana Sand Sea</rdfs:label>
    </owl:NamedIndividual>
    


    <!-- http://purl.obolibrary.org/obo/GAZ_00051200 -->

    <owl:NamedIndividual rdf:about="http://purl.obolibrary.org/obo/GAZ_00051200">
        <obo:RO_0001025 rdf:resource="http://purl.obolibrary.org/obo/GAZ_00051197"/>
        <obo:IAO_0000115>A sand sea.</obo:IAO_0000115>
        <oboInOwl:hasOBONamespace>GAZ</oboInOwl:hasOBONamespace>
        <oboInOwl:id>GAZ:00051200</oboInOwl:id>
        <rdfs:label>Egyptian Sand Sea</rdfs:label>
    </owl:NamedIndividual>
    


    <!-- http://purl.obolibrary.org/obo/GAZ_00051201 -->

    <owl:NamedIndividual rdf:about="http://purl.obolibrary.org/obo/GAZ_00051201">
        <obo:RO_0001025 rdf:resource="http://purl.obolibrary.org/obo/GAZ_00051197"/>
        <obo:IAO_0000115>A sand sea.</obo:IAO_0000115>
        <oboInOwl:hasOBONamespace>GAZ</oboInOwl:hasOBONamespace>
        <oboInOwl:id>GAZ:00051201</oboInOwl:id>
        <rdfs:label>Kalansho Sand Sea</rdfs:label>
    </owl:NamedIndividual>
    


    <!-- http://purl.obolibrary.org/obo/GAZ_00051202 -->

    <owl:NamedIndividual rdf:about="http://purl.obolibrary.org/obo/GAZ_00051202">
        <obo:RO_0001025 rdf:resource="http://purl.obolibrary.org/obo/GAZ_00051198"/>
        <obo:IAO_0000115>A dune sea that stretches from Fachi, east of the Air Mountains in north central Niger, east past the town of Bilma, on to the Chadian border. It surrounds on three sides the oasis of Bilma, southernmost of a north south string of oasies of the Kaouar rise.</obo:IAO_0000115>
        <oboInOwl:hasOBONamespace>GAZ</oboInOwl:hasOBONamespace>
        <oboInOwl:id>GAZ:00051202</oboInOwl:id>
        <rdfs:label>Erg of Bilma</rdfs:label>
    </owl:NamedIndividual>
    


    <!-- http://purl.obolibrary.org/obo/GAZ_00051203 -->

    <owl:NamedIndividual rdf:about="http://purl.obolibrary.org/obo/GAZ_00051203">
        <obo:RO_0001025 rdf:resource="http://purl.obolibrary.org/obo/GAZ_00004033"/>
        <obo:IAO_0000115>A sand sea. An that is 22 km long (North-South) and 5 km wide. Its dunes reach a maximum height of 150 meters. It is located roughly 40 km south-east of Erfoud.</obo:IAO_0000115>
        <oboInOwl:hasOBONamespace>GAZ</oboInOwl:hasOBONamespace>
        <oboInOwl:id>GAZ:00051203</oboInOwl:id>
        <rdfs:label>Erg Chebbi</rdfs:label>
    </owl:NamedIndividual>
    


    <!-- http://purl.obolibrary.org/obo/GAZ_00052553 -->

    <owl:NamedIndividual rdf:about="http://purl.obolibrary.org/obo/GAZ_00052553">
        <obo:IAO_0000115>A river that rises in the central highlands of Ethiopia near Mount Qachen, from where it flows west, north, then west again, forming the westernmost border of Ethiopia and Eritrea. The river continues into northeastern Sudan, where at 14deg10minN, 36degE, the Tekeze joins the Atbarah River, the lower course of which is a tributary of the Nile. The Tekeze is perhaps the true upper course of the Atbarah, as the former follows the longer course prior to the confluence of the two rivers. The names of its main tributaries in Ethiopia from its source are: on the right bank Tahali, Meri, Sellare, Sullo, Arekwa, Gheoa, Wari, Firafira, Tocoro and Gumalo Rivers; on the left bank Nili, Balagas, Saha, Bembea, Ataba, Zarima, and Kwalema Rivers.</obo:IAO_0000115>
        <oboInOwl:hasOBONamespace>GAZ</oboInOwl:hasOBONamespace>
        <oboInOwl:id>GAZ:00052553</oboInOwl:id>
        <rdfs:label>Tekeze River</rdfs:label>
    </owl:NamedIndividual>
    


    <!-- http://purl.obolibrary.org/obo/GAZ_00053489 -->

    <owl:NamedIndividual rdf:about="http://purl.obolibrary.org/obo/GAZ_00053489">
        <obo:RO_0001025 rdf:resource="http://purl.obolibrary.org/obo/GAZ_00103898"/>
        <obo:IAO_0000115>A volcanic field covers a broad area of about 1050 km2 in the Tuareg shield in the southern Air region of Niger. Activity began with the eruption of about 30 trachytic and phonolitic volcanoes through Precambrian basement rocks. This was followed by the formation of about 130 basaltic cones that typically produced a valley filling lava flow. A series of NW-SE-trending faults control volcano locations.</obo:IAO_0000115>
        <oboInOwl:hasOBONamespace>GAZ</oboInOwl:hasOBONamespace>
        <oboInOwl:id>GAZ:00053489</oboInOwl:id>
        <rdfs:label>Todra Volcanic Field</rdfs:label>
    </owl:NamedIndividual>
    


    <!-- http://purl.obolibrary.org/obo/GAZ_00053491 -->

    <owl:NamedIndividual rdf:about="http://purl.obolibrary.org/obo/GAZ_00053491">
        <obo:RO_0001025 rdf:resource="http://purl.obolibrary.org/obo/GAZ_00000822"/>
        <obo:IAO_0000115>A volcanic field (pyroclastic cones) that lies in SE Algeria, near the border with Niger. The alkaline In Ezzane volcanic field, part of which extends into Niger, covers about 500 km2 at the eastern end of Hoggar (Ahaggar) volcanic province and was assigned a Recent age.</obo:IAO_0000115>
        <oboInOwl:hasOBONamespace>GAZ</oboInOwl:hasOBONamespace>
        <oboInOwl:id>GAZ:00053491</oboInOwl:id>
        <rdfs:label>In Ezzane Volcanic Field</rdfs:label>
    </owl:NamedIndividual>
    


    <!-- http://purl.obolibrary.org/obo/GAZ_00053496 -->

    <owl:NamedIndividual rdf:about="http://purl.obolibrary.org/obo/GAZ_00053496">
        <obo:IAO_0000115>A volcanic field that lies in the Sahara desert of south-central Libya, south of the Haruj volcanic field. A 4 km wide, 100-m-deep caldera contains a post-caldera scoria cone, Wau-en-Namus. An apron of dark basaltic tephra extends 10-20 km around the caldera in stark contrast to the light-colored desert sand prominent in satellite views. Three small saline lakes of variable color contribute to the name of the volcano.</obo:IAO_0000115>
        <oboInOwl:hasOBONamespace>GAZ</oboInOwl:hasOBONamespace>
        <oboInOwl:id>GAZ:00053496</oboInOwl:id>
        <rdfs:label>Wau-en-Namus Volcanic Field</rdfs:label>
    </owl:NamedIndividual>
    


    <!-- http://purl.obolibrary.org/obo/GAZ_00053509 -->

    <owl:NamedIndividual rdf:about="http://purl.obolibrary.org/obo/GAZ_00053509">
        <obo:RO_0001025 rdf:resource="http://purl.obolibrary.org/obo/GAZ_00057756"/>
        <obo:IAO_0000115>A volcanic field is located in the Bayuda Desert of NE Sudan, south of the major Abu Hamed bend of the Nile River about 300 km north of capital city of Khartoum. More than 90 eruptive centers along a WNW-ESE line were constructed over Precambrian and Paleozoic granitic rocks near the center of the Bayuda Desert. Most vents of the Bayuda field are cinder cones that produced lava flows which breached the cones. About 10% of vents in the field are explosion craters, the largest of which, named Hosh ed Dalam, is 1.3 km wide and up to 500 m deep.</obo:IAO_0000115>
        <oboInOwl:hasOBONamespace>GAZ</oboInOwl:hasOBONamespace>
        <oboInOwl:id>GAZ:00053509</oboInOwl:id>
        <rdfs:label>Bayuda Volcanic Field</rdfs:label>
    </owl:NamedIndividual>
    


    <!-- http://purl.obolibrary.org/obo/GAZ_00053510 -->

    <owl:NamedIndividual rdf:about="http://purl.obolibrary.org/obo/GAZ_00053510">
        <obo:RO_0001025 rdf:resource="http://purl.obolibrary.org/obo/GAZ_00053509"/>
        <obo:IAO_0000115>A volanic crater.</obo:IAO_0000115>
        <oboInOwl:hasOBONamespace>GAZ</oboInOwl:hasOBONamespace>
        <oboInOwl:id>GAZ:00053510</oboInOwl:id>
        <rdfs:label>Hosh ed Dalam</rdfs:label>
    </owl:NamedIndividual>
    


    <!-- http://purl.obolibrary.org/obo/GAZ_00053511 -->

    <owl:NamedIndividual rdf:about="http://purl.obolibrary.org/obo/GAZ_00053511">
        <obo:RO_0001025 rdf:resource="http://purl.obolibrary.org/obo/GAZ_00057756"/>
        <obo:IAO_0000115>A volcanic field (shield volcano) located in the Bayuda desert of NE Sudan, immediately west of the Nile River, NE of the capital city of Khartoum. Jebel Umm Arafieb consists of a low-angle shield volcano of basanitic-to-trachybasaltic composition formed of several overlapping aa lava flows erupted from a vent now capped by a spatter cone.</obo:IAO_0000115>
        <oboInOwl:hasOBONamespace>GAZ</oboInOwl:hasOBONamespace>
        <oboInOwl:id>GAZ:00053511</oboInOwl:id>
        <rdfs:label>Jebel Umm Arafieb Volcanic Field</rdfs:label>
    </owl:NamedIndividual>
    


    <!-- http://purl.obolibrary.org/obo/GAZ_00057756 -->

    <owl:NamedIndividual rdf:about="http://purl.obolibrary.org/obo/GAZ_00057756">
        <obo:IAO_0000115>A desert located north of Khartoum, Sudan, west of Kadabas, and north of the Nubian Desert, together making up part of the Sahara&apos;s eastern flank.</obo:IAO_0000115>
        <oboInOwl:hasOBONamespace>GAZ</oboInOwl:hasOBONamespace>
        <oboInOwl:id>GAZ:00057756</oboInOwl:id>
        <rdfs:label>Bayuda Desert</rdfs:label>
    </owl:NamedIndividual>
    


    <!-- http://purl.obolibrary.org/obo/GAZ_00057757 -->

    <owl:NamedIndividual rdf:about="http://purl.obolibrary.org/obo/GAZ_00057757">
        <obo:IAO_0000115>The eastern region of the Sahara Desert, it spans 50, 000 km2 of northeastern Sudan between the Nile and the Red Sea.</obo:IAO_0000115>
        <oboInOwl:hasOBONamespace>GAZ</oboInOwl:hasOBONamespace>
        <oboInOwl:id>GAZ:00057757</oboInOwl:id>
        <rdfs:label>Nubian Desert</rdfs:label>
    </owl:NamedIndividual>
    


    <!-- http://purl.obolibrary.org/obo/GAZ_00057759 -->

    <owl:NamedIndividual rdf:about="http://purl.obolibrary.org/obo/GAZ_00057759">
        <obo:IAO_0000115>A desert east of the river Nile, between the Nile and the Red Sea. It extends from Egypt in the north to Eritrea in the south, and also comprises parts of Sudan and Ethiopia.</obo:IAO_0000115>
        <oboInOwl:hasOBONamespace>GAZ</oboInOwl:hasOBONamespace>
        <oboInOwl:id>GAZ:00057759</oboInOwl:id>
        <rdfs:label>Eastern Desert</rdfs:label>
    </owl:NamedIndividual>
    


    <!-- http://purl.obolibrary.org/obo/GAZ_00058791 -->

    <owl:NamedIndividual rdf:about="http://purl.obolibrary.org/obo/GAZ_00058791">
        <obo:IAO_0000115>A polymictic shallow lake complex of Uganda, about 1,720 km2 in area and at an elevation of 914 m. The Victoria Nile flows through the lake on its way from Lake Victoria to Lake Albert. The main inflow from Lake Victoria is regulated by the Nalubaale Power Station in Jinja. Another source of water is the Mount Elgon region on the border between Uganda and Kenya.</obo:IAO_0000115>
        <oboInOwl:hasOBONamespace>GAZ</oboInOwl:hasOBONamespace>
        <oboInOwl:id>GAZ:00058791</oboInOwl:id>
        <rdfs:label>Lake Kyoga</rdfs:label>
    </owl:NamedIndividual>
    


    <!-- http://purl.obolibrary.org/obo/GAZ_00058824 -->

    <owl:NamedIndividual rdf:about="http://purl.obolibrary.org/obo/GAZ_00058824">
        <obo:IAO_0000115>A reservoir on the Niger River, formed by the Kainji Dam. It is a part of Niger State and Kebbi State. Constructed 1968.</obo:IAO_0000115>
        <oboInOwl:hasOBONamespace>GAZ</oboInOwl:hasOBONamespace>
        <oboInOwl:id>GAZ:00058824</oboInOwl:id>
        <rdfs:label>Kainji Lake</rdfs:label>
    </owl:NamedIndividual>
    


    <!-- http://purl.obolibrary.org/obo/GAZ_00058829 -->

    <owl:NamedIndividual rdf:about="http://purl.obolibrary.org/obo/GAZ_00058829">
        <obo:RO_0001025 rdf:resource="http://purl.obolibrary.org/obo/GAZ_00147864"/>
        <obo:IAO_0000115>A lake in central part of Mali.</obo:IAO_0000115>
        <oboInOwl:hasOBONamespace>GAZ</oboInOwl:hasOBONamespace>
        <oboInOwl:id>GAZ:00058829</oboInOwl:id>
        <rdfs:label>Lake Debo</rdfs:label>
    </owl:NamedIndividual>
    


    <!-- http://purl.obolibrary.org/obo/GAZ_00058849 -->

    <owl:NamedIndividual rdf:about="http://purl.obolibrary.org/obo/GAZ_00058849">
        <obo:RO_0001025 rdf:resource="http://purl.obolibrary.org/obo/GAZ_00051197"/>
        <obo:IAO_0000115>Recently formed endorheic lakes in the Sahara Desert of Egypt. Caused by water from Lake Nasser running through the Sadat Canal.</obo:IAO_0000115>
        <oboInOwl:hasOBONamespace>GAZ</oboInOwl:hasOBONamespace>
        <oboInOwl:id>GAZ:00058849</oboInOwl:id>
        <rdfs:label>Toshka Lakes</rdfs:label>
    </owl:NamedIndividual>
    


    <!-- http://purl.obolibrary.org/obo/GAZ_00058861 -->

    <owl:NamedIndividual rdf:about="http://purl.obolibrary.org/obo/GAZ_00058861">
        <obo:IAO_0000115>An island in Lake Chad.</obo:IAO_0000115>
        <oboInOwl:hasOBONamespace>GAZ</oboInOwl:hasOBONamespace>
        <oboInOwl:id>GAZ:00058861</oboInOwl:id>
        <rdfs:label>Tebour Island</rdfs:label>
    </owl:NamedIndividual>
    


    <!-- http://purl.obolibrary.org/obo/GAZ_00058862 -->

    <owl:NamedIndividual rdf:about="http://purl.obolibrary.org/obo/GAZ_00058862">
        <obo:IAO_0000115>An island in Lake Chad.</obo:IAO_0000115>
        <oboInOwl:hasOBONamespace>GAZ</oboInOwl:hasOBONamespace>
        <oboInOwl:id>GAZ:00058862</oboInOwl:id>
        <rdfs:label>Isseirom Island</rdfs:label>
    </owl:NamedIndividual>
    


    <!-- http://purl.obolibrary.org/obo/GAZ_00058863 -->

    <owl:NamedIndividual rdf:about="http://purl.obolibrary.org/obo/GAZ_00058863">
        <obo:IAO_0000115>An island in Lake Chad.</obo:IAO_0000115>
        <oboInOwl:hasOBONamespace>GAZ</oboInOwl:hasOBONamespace>
        <oboInOwl:id>GAZ:00058863</oboInOwl:id>
        <rdfs:label>Malal Island</rdfs:label>
    </owl:NamedIndividual>
    


    <!-- http://purl.obolibrary.org/obo/GAZ_00058864 -->

    <owl:NamedIndividual rdf:about="http://purl.obolibrary.org/obo/GAZ_00058864">
        <obo:IAO_0000115>An island in Lake Chad.</obo:IAO_0000115>
        <oboInOwl:hasOBONamespace>GAZ</oboInOwl:hasOBONamespace>
        <oboInOwl:id>GAZ:00058864</oboInOwl:id>
        <rdfs:label>Ngelea Island</rdfs:label>
    </owl:NamedIndividual>
    


    <!-- http://purl.obolibrary.org/obo/GAZ_00058865 -->

    <owl:NamedIndividual rdf:about="http://purl.obolibrary.org/obo/GAZ_00058865">
        <obo:IAO_0000115>An island in Lake Chad.</obo:IAO_0000115>
        <oboInOwl:hasOBONamespace>GAZ</oboInOwl:hasOBONamespace>
        <oboInOwl:id>GAZ:00058865</oboInOwl:id>
        <rdfs:label>Kofia Island</rdfs:label>
    </owl:NamedIndividual>
    


    <!-- http://purl.obolibrary.org/obo/GAZ_00058866 -->

    <owl:NamedIndividual rdf:about="http://purl.obolibrary.org/obo/GAZ_00058866">
        <obo:IAO_0000115>An island in Lake Chad.</obo:IAO_0000115>
        <oboInOwl:hasOBONamespace>GAZ</oboInOwl:hasOBONamespace>
        <oboInOwl:id>GAZ:00058866</oboInOwl:id>
        <rdfs:label>Kindjera Island</rdfs:label>
    </owl:NamedIndividual>
    


    <!-- http://purl.obolibrary.org/obo/GAZ_00058867 -->

    <owl:NamedIndividual rdf:about="http://purl.obolibrary.org/obo/GAZ_00058867">
        <obo:IAO_0000115>An island in Lake Chad.</obo:IAO_0000115>
        <oboInOwl:hasOBONamespace>GAZ</oboInOwl:hasOBONamespace>
        <oboInOwl:id>GAZ:00058867</oboInOwl:id>
        <rdfs:label>Kalom Island</rdfs:label>
    </owl:NamedIndividual>
    


    <!-- http://purl.obolibrary.org/obo/GAZ_00058868 -->

    <owl:NamedIndividual rdf:about="http://purl.obolibrary.org/obo/GAZ_00058868">
        <obo:IAO_0000115>An island in Lake Chad.</obo:IAO_0000115>
        <oboInOwl:hasOBONamespace>GAZ</oboInOwl:hasOBONamespace>
        <oboInOwl:id>GAZ:00058868</oboInOwl:id>
        <rdfs:label>Dabouroum Island</rdfs:label>
    </owl:NamedIndividual>
    


    <!-- http://purl.obolibrary.org/obo/GAZ_00058869 -->

    <owl:NamedIndividual rdf:about="http://purl.obolibrary.org/obo/GAZ_00058869">
        <obo:IAO_0000115>An island in Lake Chad.</obo:IAO_0000115>
        <oboInOwl:hasOBONamespace>GAZ</oboInOwl:hasOBONamespace>
        <oboInOwl:id>GAZ:00058869</oboInOwl:id>
        <rdfs:label>Kika Island</rdfs:label>
    </owl:NamedIndividual>
    


    <!-- http://purl.obolibrary.org/obo/GAZ_00058872 -->

    <owl:NamedIndividual rdf:about="http://purl.obolibrary.org/obo/GAZ_00058872">
        <obo:IAO_0000115>The two dams at the first cataract on the Nile in Egypt.</obo:IAO_0000115>
        <oboInOwl:hasOBONamespace>GAZ</oboInOwl:hasOBONamespace>
        <oboInOwl:id>GAZ:00058872</oboInOwl:id>
        <rdfs:label>Aswan Dams</rdfs:label>
    </owl:NamedIndividual>
    


    <!-- http://purl.obolibrary.org/obo/GAZ_00058873 -->

    <owl:NamedIndividual rdf:about="http://purl.obolibrary.org/obo/GAZ_00058873">
        <obo:RO_0001025 rdf:resource="http://purl.obolibrary.org/obo/GAZ_00058872"/>
        <obo:IAO_0000115>The newer of the Aswan Dams, completed in 1968. It is located 7 km south of Aswan City.</obo:IAO_0000115>
        <oboInOwl:hasOBONamespace>GAZ</oboInOwl:hasOBONamespace>
        <oboInOwl:id>GAZ:00058873</oboInOwl:id>
        <rdfs:label>Aswan High Dam</rdfs:label>
    </owl:NamedIndividual>
    


    <!-- http://purl.obolibrary.org/obo/GAZ_00058874 -->

    <owl:NamedIndividual rdf:about="http://purl.obolibrary.org/obo/GAZ_00058874">
        <obo:RO_0001025 rdf:resource="http://purl.obolibrary.org/obo/GAZ_00058872"/>
        <obo:IAO_0000115>The first of the Aswan Dams on the Nile, finished in 1902.</obo:IAO_0000115>
        <oboInOwl:hasOBONamespace>GAZ</oboInOwl:hasOBONamespace>
        <oboInOwl:id>GAZ:00058874</oboInOwl:id>
        <rdfs:label>Aswan Low Dam</rdfs:label>
    </owl:NamedIndividual>
    


    <!-- http://purl.obolibrary.org/obo/GAZ_00058877 -->

    <owl:NamedIndividual rdf:about="http://purl.obolibrary.org/obo/GAZ_00058877">
        <obo:RO_0001025 rdf:resource="http://purl.obolibrary.org/obo/GAZ_00009949"/>
        <obo:IAO_0000115>A dam that was completed in 1862. Its purpose was to improve irrigation in the Nile Delta area of Egypt.</obo:IAO_0000115>
        <oboInOwl:hasOBONamespace>GAZ</oboInOwl:hasOBONamespace>
        <oboInOwl:id>GAZ:00058877</oboInOwl:id>
        <rdfs:label>Delta Barrage</rdfs:label>
    </owl:NamedIndividual>
    


    <!-- http://purl.obolibrary.org/obo/GAZ_00058878 -->

    <owl:NamedIndividual rdf:about="http://purl.obolibrary.org/obo/GAZ_00058878">
        <rdf:type rdf:resource="http://purl.obolibrary.org/obo/ENVO_00000074"/>
        <obo:IAO_0000115>A barrage on the River Nile in Egypt.</obo:IAO_0000115>
        <oboInOwl:hasOBONamespace>GAZ</oboInOwl:hasOBONamespace>
        <oboInOwl:id>GAZ:00058878</oboInOwl:id>
        <rdfs:label>Esna Barrage</rdfs:label>
    </owl:NamedIndividual>
    


    <!-- http://purl.obolibrary.org/obo/GAZ_00058879 -->

    <owl:NamedIndividual rdf:about="http://purl.obolibrary.org/obo/GAZ_00058879">
        <rdf:type rdf:resource="http://purl.obolibrary.org/obo/ENVO_00000074"/>
        <obo:IAO_0000115>A barrage on the River Nile in Egypt.</obo:IAO_0000115>
        <oboInOwl:hasOBONamespace>GAZ</oboInOwl:hasOBONamespace>
        <oboInOwl:id>GAZ:00058879</oboInOwl:id>
        <rdfs:label>Nag Hammadi Barrage</rdfs:label>
    </owl:NamedIndividual>
    


    <!-- http://purl.obolibrary.org/obo/GAZ_00058880 -->

    <owl:NamedIndividual rdf:about="http://purl.obolibrary.org/obo/GAZ_00058880">
        <rdf:type rdf:resource="http://purl.obolibrary.org/obo/ENVO_00000074"/>
        <obo:IAO_0000115>A barrage on the River Nile in Egypt.</obo:IAO_0000115>
        <oboInOwl:hasOBONamespace>GAZ</oboInOwl:hasOBONamespace>
        <oboInOwl:id>GAZ:00058880</oboInOwl:id>
        <rdfs:label>Assuit Barrage</rdfs:label>
    </owl:NamedIndividual>
    


    <!-- http://purl.obolibrary.org/obo/GAZ_00058881 -->

    <owl:NamedIndividual rdf:about="http://purl.obolibrary.org/obo/GAZ_00058881">
        <obo:IAO_0000115>A dam on the Rosetta Canal.</obo:IAO_0000115>
        <oboInOwl:hasOBONamespace>GAZ</oboInOwl:hasOBONamespace>
        <oboInOwl:id>GAZ:00058881</oboInOwl:id>
        <rdfs:label>Edfina Barrage</rdfs:label>
    </owl:NamedIndividual>
    


    <!-- http://purl.obolibrary.org/obo/GAZ_00058882 -->

    <owl:NamedIndividual rdf:about="http://purl.obolibrary.org/obo/GAZ_00058882">
        <obo:IAO_0000115>A dam on the Damietta Canal.</obo:IAO_0000115>
        <oboInOwl:hasOBONamespace>GAZ</oboInOwl:hasOBONamespace>
        <oboInOwl:id>GAZ:00058882</oboInOwl:id>
        <rdfs:label>Faraskour Barrage</rdfs:label>
    </owl:NamedIndividual>
    


    <!-- http://purl.obolibrary.org/obo/GAZ_00058883 -->

    <owl:NamedIndividual rdf:about="http://purl.obolibrary.org/obo/GAZ_00058883">
        <obo:IAO_0000115>A dam on the Damietta Canal.</obo:IAO_0000115>
        <oboInOwl:hasOBONamespace>GAZ</oboInOwl:hasOBONamespace>
        <oboInOwl:id>GAZ:00058883</oboInOwl:id>
        <rdfs:label>Zitta Barrage</rdfs:label>
    </owl:NamedIndividual>
    


    <!-- http://purl.obolibrary.org/obo/GAZ_00058884 -->

    <owl:NamedIndividual rdf:about="http://purl.obolibrary.org/obo/GAZ_00058884"/>
    


    <!-- http://purl.obolibrary.org/obo/GAZ_00058886 -->

    <owl:NamedIndividual rdf:about="http://purl.obolibrary.org/obo/GAZ_00058886"/>
    


    <!-- http://purl.obolibrary.org/obo/GAZ_00058890 -->

    <owl:NamedIndividual rdf:about="http://purl.obolibrary.org/obo/GAZ_00058890"/>
    


    <!-- http://purl.obolibrary.org/obo/GAZ_00058891 -->

    <owl:NamedIndividual rdf:about="http://purl.obolibrary.org/obo/GAZ_00058891">
        <obo:RO_0001025 rdf:resource="http://purl.obolibrary.org/obo/GAZ_00058886"/>
        <obo:IAO_0000115>An island in the River Nile in Egypt near the Fourth Cataract in Dar al-Manasir.</obo:IAO_0000115>
        <oboInOwl:hasOBONamespace>GAZ</oboInOwl:hasOBONamespace>
        <oboInOwl:id>GAZ:00058891</oboInOwl:id>
        <rdfs:label>Island of Muqrat</rdfs:label>
    </owl:NamedIndividual>
    


    <!-- http://purl.obolibrary.org/obo/GAZ_00058892 -->

    <owl:NamedIndividual rdf:about="http://purl.obolibrary.org/obo/GAZ_00058892">
        <obo:IAO_0000115>A dam under construction on the River Nile in Sudan, about 350 km north of the capital Khartoum.</obo:IAO_0000115>
        <oboInOwl:hasOBONamespace>GAZ</oboInOwl:hasOBONamespace>
        <oboInOwl:id>GAZ:00058892</oboInOwl:id>
        <rdfs:label>Merowe High Dam</rdfs:label>
    </owl:NamedIndividual>
    


    <!-- http://purl.obolibrary.org/obo/GAZ_00066409 -->

    <owl:NamedIndividual rdf:about="http://purl.obolibrary.org/obo/GAZ_00066409">
        <obo:RO_0001025 rdf:resource="http://purl.obolibrary.org/obo/GAZ_00248009"/>
        <obo:IAO_0000115>An oasis in Egypt, located between the Qattara Depression and the Egyptian Sand Sea in the Libyan Desert, nearly 50 km east of the Libyan border, and 560 km from Cairo.</obo:IAO_0000115>
        <oboInOwl:hasOBONamespace>GAZ</oboInOwl:hasOBONamespace>
        <oboInOwl:id>GAZ:00066409</oboInOwl:id>
        <rdfs:label>Siwa Oasis</rdfs:label>
    </owl:NamedIndividual>
    


    <!-- http://purl.obolibrary.org/obo/GAZ_00066410 -->

    <owl:NamedIndividual rdf:about="http://purl.obolibrary.org/obo/GAZ_00066410">
        <obo:RO_0001025 rdf:resource="http://purl.obolibrary.org/obo/GAZ_00051197"/>
        <obo:IAO_0000115>A desert located 45 km north of Farafra. The desert has a white, cream color and has massive chalk rock formations that have been created as a result of occasional sandstorms in the area.</obo:IAO_0000115>
        <oboInOwl:hasOBONamespace>GAZ</oboInOwl:hasOBONamespace>
        <oboInOwl:id>GAZ:00066410</oboInOwl:id>
        <rdfs:label>Sahara el Beyda</rdfs:label>
    </owl:NamedIndividual>
    


    <!-- http://purl.obolibrary.org/obo/GAZ_00066428 -->

    <owl:NamedIndividual rdf:about="http://purl.obolibrary.org/obo/GAZ_00066428">
        <obo:RO_0001025 rdf:resource="http://purl.obolibrary.org/obo/GAZ_00051197"/>
        <obo:IAO_0000115>An oasis with a large lake located in the municipality Sabha in the Libyan Sahara. The lake is saline.</obo:IAO_0000115>
        <oboInOwl:hasOBONamespace>GAZ</oboInOwl:hasOBONamespace>
        <oboInOwl:id>GAZ:00066428</oboInOwl:id>
        <rdfs:label>Gaberoun Oasis</rdfs:label>
    </owl:NamedIndividual>
    


    <!-- http://purl.obolibrary.org/obo/GAZ_00066429 -->

    <owl:NamedIndividual rdf:about="http://purl.obolibrary.org/obo/GAZ_00066429">
        <obo:RO_0001025 rdf:resource="http://purl.obolibrary.org/obo/GAZ_00051197"/>
        <obo:IAO_0000115>An erg.</obo:IAO_0000115>
        <oboInOwl:hasOBONamespace>GAZ</oboInOwl:hasOBONamespace>
        <oboInOwl:id>GAZ:00066429</oboInOwl:id>
        <rdfs:label>Ramlat al Dauada</rdfs:label>
    </owl:NamedIndividual>
    


    <!-- http://purl.obolibrary.org/obo/GAZ_00066430 -->

    <owl:NamedIndividual rdf:about="http://purl.obolibrary.org/obo/GAZ_00066430">
        <obo:RO_0001025 rdf:resource="http://purl.obolibrary.org/obo/GAZ_00066429"/>
        <obo:IAO_0000115>A lake in the Ramlat al Dauada erg.</obo:IAO_0000115>
        <oboInOwl:hasOBONamespace>GAZ</oboInOwl:hasOBONamespace>
        <oboInOwl:id>GAZ:00066430</oboInOwl:id>
        <rdfs:label>Mafo Lake</rdfs:label>
    </owl:NamedIndividual>
    


    <!-- http://purl.obolibrary.org/obo/GAZ_00066431 -->

    <owl:NamedIndividual rdf:about="http://purl.obolibrary.org/obo/GAZ_00066431">
        <obo:RO_0001025 rdf:resource="http://purl.obolibrary.org/obo/GAZ_00051197"/>
        <obo:IAO_0000115>An oasis in Southeastern Libya.</obo:IAO_0000115>
        <oboInOwl:hasOBONamespace>GAZ</oboInOwl:hasOBONamespace>
        <oboInOwl:id>GAZ:00066431</oboInOwl:id>
        <rdfs:label>Kufra Oasis</rdfs:label>
    </owl:NamedIndividual>
    


    <!-- http://purl.obolibrary.org/obo/GAZ_00089782 -->

    <owl:NamedIndividual rdf:about="http://purl.obolibrary.org/obo/GAZ_00089782">
        <obo:IAO_0000115>Protected areas amounting to 144 islands in different Governorates in Egypt. Alongside the main stream from Aswan until the Barrages, there are 95 Islands within an area of 32500 Feddans. In Rasheed branch there are 30 islands within an area of 3400 Feddans, in Damietta Branch there are 19 islands within and area of 1250 Feddans. The total area of all the Nile River islands in 37150 Feddans.</obo:IAO_0000115>
        <oboInOwl:hasOBONamespace>GAZ</oboInOwl:hasOBONamespace>
        <oboInOwl:id>GAZ:00089782</oboInOwl:id>
        <rdfs:label>Nile river Islands Protected Area</rdfs:label>
    </owl:NamedIndividual>
    


    <!-- http://purl.obolibrary.org/obo/GAZ_00103898 -->

    <owl:NamedIndividual rdf:about="http://purl.obolibrary.org/obo/GAZ_00103898">
        <obo:RO_0001025 rdf:resource="http://purl.obolibrary.org/obo/GAZ_00000585"/>
        <obo:IAO_0000115>A triangular massif, located in northern Niger, within the Sahara desert. Part of the West Saharan montane xeric woodlands ecoregion, they rise to more than 1,830 m and extend over 84000 km2. Lying in the midst of desert north of the 17th parallel, the Air plateau with an average altitude between 500 and 900 m, forms an island of Sahel climate.</obo:IAO_0000115>
        <oboInOwl:hasOBONamespace>GAZ</oboInOwl:hasOBONamespace>
        <oboInOwl:id>GAZ:00103898</oboInOwl:id>
        <rdfs:label>Air Mountains</rdfs:label>
    </owl:NamedIndividual>
    


    <!-- http://purl.obolibrary.org/obo/GAZ_00113893 -->

    <owl:NamedIndividual rdf:about="http://purl.obolibrary.org/obo/GAZ_00113893">
        <obo:RO_0001025 rdf:resource="http://purl.obolibrary.org/obo/GAZ_00000828"/>
        <oboInOwl:hasOBONamespace>GAZ</oboInOwl:hasOBONamespace>
        <oboInOwl:id>GAZ:00113893</oboInOwl:id>
        <rdfs:label>Communaute Urbaine de Zinder</rdfs:label>
    </owl:NamedIndividual>
    


    <!-- http://purl.obolibrary.org/obo/GAZ_00113936 -->

    <owl:NamedIndividual rdf:about="http://purl.obolibrary.org/obo/GAZ_00113936">
        <obo:RO_0001025 rdf:resource="http://purl.obolibrary.org/obo/GAZ_00113893"/>
        <oboInOwl:hasOBONamespace>GAZ</oboInOwl:hasOBONamespace>
        <oboInOwl:id>GAZ:00113936</oboInOwl:id>
        <rdfs:label>Commune of Zinder II</rdfs:label>
    </owl:NamedIndividual>
    


    <!-- http://purl.obolibrary.org/obo/GAZ_00113937 -->

    <owl:NamedIndividual rdf:about="http://purl.obolibrary.org/obo/GAZ_00113937">
        <obo:RO_0001025 rdf:resource="http://purl.obolibrary.org/obo/GAZ_00113893"/>
        <oboInOwl:hasOBONamespace>GAZ</oboInOwl:hasOBONamespace>
        <oboInOwl:id>GAZ:00113937</oboInOwl:id>
        <rdfs:label>Commune of Zinder IV</rdfs:label>
    </owl:NamedIndividual>
    


    <!-- http://purl.obolibrary.org/obo/GAZ_00113938 -->

    <owl:NamedIndividual rdf:about="http://purl.obolibrary.org/obo/GAZ_00113938">
        <obo:RO_0001025 rdf:resource="http://purl.obolibrary.org/obo/GAZ_00113893"/>
        <oboInOwl:hasOBONamespace>GAZ</oboInOwl:hasOBONamespace>
        <oboInOwl:id>GAZ:00113938</oboInOwl:id>
        <rdfs:label>Commune of Zinder I</rdfs:label>
    </owl:NamedIndividual>
    


    <!-- http://purl.obolibrary.org/obo/GAZ_00113939 -->

    <owl:NamedIndividual rdf:about="http://purl.obolibrary.org/obo/GAZ_00113939">
        <obo:RO_0001025 rdf:resource="http://purl.obolibrary.org/obo/GAZ_00113893"/>
        <oboInOwl:hasOBONamespace>GAZ</oboInOwl:hasOBONamespace>
        <oboInOwl:id>GAZ:00113939</oboInOwl:id>
        <rdfs:label>Commune of Zinder III</rdfs:label>
    </owl:NamedIndividual>
    


    <!-- http://purl.obolibrary.org/obo/GAZ_00113940 -->

    <owl:NamedIndividual rdf:about="http://purl.obolibrary.org/obo/GAZ_00113940">
        <obo:RO_0001025 rdf:resource="http://purl.obolibrary.org/obo/GAZ_00113893"/>
        <oboInOwl:hasOBONamespace>GAZ</oboInOwl:hasOBONamespace>
        <oboInOwl:id>GAZ:00113940</oboInOwl:id>
        <rdfs:label>Commune of Zinder V</rdfs:label>
    </owl:NamedIndividual>
    


    <!-- http://purl.obolibrary.org/obo/GAZ_00113941 -->

    <owl:NamedIndividual rdf:about="http://purl.obolibrary.org/obo/GAZ_00113941">
        <obo:RO_0001025 rdf:resource="http://purl.obolibrary.org/obo/GAZ_00032140"/>
        <obo:IAO_0000115>A commune of Tillaberi Department, Niger.</obo:IAO_0000115>
        <oboInOwl:hasOBONamespace>GAZ</oboInOwl:hasOBONamespace>
        <oboInOwl:id>GAZ:00113941</oboInOwl:id>
        <rdfs:label>Commune of Anzourou</rdfs:label>
    </owl:NamedIndividual>
    


    <!-- http://purl.obolibrary.org/obo/GAZ_00113942 -->

    <owl:NamedIndividual rdf:about="http://purl.obolibrary.org/obo/GAZ_00113942">
        <obo:RO_0001025 rdf:resource="http://purl.obolibrary.org/obo/GAZ_00032140"/>
        <obo:IAO_0000115>A commune of Tillaberi Department, Niger.</obo:IAO_0000115>
        <oboInOwl:hasOBONamespace>GAZ</oboInOwl:hasOBONamespace>
        <oboInOwl:id>GAZ:00113942</oboInOwl:id>
        <rdfs:label>Commune of Ayorou</rdfs:label>
    </owl:NamedIndividual>
    


    <!-- http://purl.obolibrary.org/obo/GAZ_00113943 -->

    <owl:NamedIndividual rdf:about="http://purl.obolibrary.org/obo/GAZ_00113943">
        <obo:RO_0001025 rdf:resource="http://purl.obolibrary.org/obo/GAZ_00032140"/>
        <obo:IAO_0000115>A commune of Tillaberi Department, Niger.</obo:IAO_0000115>
        <oboInOwl:hasOBONamespace>GAZ</oboInOwl:hasOBONamespace>
        <oboInOwl:id>GAZ:00113943</oboInOwl:id>
        <rdfs:label>Commune of Sinder</rdfs:label>
    </owl:NamedIndividual>
    


    <!-- http://purl.obolibrary.org/obo/GAZ_00113944 -->

    <owl:NamedIndividual rdf:about="http://purl.obolibrary.org/obo/GAZ_00113944">
        <obo:RO_0001025 rdf:resource="http://purl.obolibrary.org/obo/GAZ_00032140"/>
        <obo:IAO_0000115>A commune of Tillaberi Department, Niger.</obo:IAO_0000115>
        <oboInOwl:hasOBONamespace>GAZ</oboInOwl:hasOBONamespace>
        <oboInOwl:id>GAZ:00113944</oboInOwl:id>
        <rdfs:label>Commune of Dessa</rdfs:label>
    </owl:NamedIndividual>
    


    <!-- http://purl.obolibrary.org/obo/GAZ_00113945 -->

    <owl:NamedIndividual rdf:about="http://purl.obolibrary.org/obo/GAZ_00113945">
        <obo:RO_0001025 rdf:resource="http://purl.obolibrary.org/obo/GAZ_00032140"/>
        <obo:IAO_0000115>A commune of Tillaberi Department, Niger.</obo:IAO_0000115>
        <oboInOwl:hasOBONamespace>GAZ</oboInOwl:hasOBONamespace>
        <oboInOwl:id>GAZ:00113945</oboInOwl:id>
        <rdfs:label>Commune of Kourteye</rdfs:label>
    </owl:NamedIndividual>
    


    <!-- http://purl.obolibrary.org/obo/GAZ_00113946 -->

    <owl:NamedIndividual rdf:about="http://purl.obolibrary.org/obo/GAZ_00113946">
        <obo:RO_0001025 rdf:resource="http://purl.obolibrary.org/obo/GAZ_00032140"/>
        <obo:IAO_0000115>A commune of Tillaberi Department, Niger.</obo:IAO_0000115>
        <oboInOwl:hasOBONamespace>GAZ</oboInOwl:hasOBONamespace>
        <oboInOwl:id>GAZ:00113946</oboInOwl:id>
        <rdfs:label>Communaute Urbaine de Tillaberi</rdfs:label>
    </owl:NamedIndividual>
    


    <!-- http://purl.obolibrary.org/obo/GAZ_00113947 -->

    <owl:NamedIndividual rdf:about="http://purl.obolibrary.org/obo/GAZ_00113947">
        <obo:RO_0001025 rdf:resource="http://purl.obolibrary.org/obo/GAZ_00032140"/>
        <obo:IAO_0000115>A commune of Tillaberi Department, Niger.</obo:IAO_0000115>
        <oboInOwl:hasOBONamespace>GAZ</oboInOwl:hasOBONamespace>
        <oboInOwl:id>GAZ:00113947</oboInOwl:id>
        <rdfs:label>Commune of Sakoira</rdfs:label>
    </owl:NamedIndividual>
    


    <!-- http://purl.obolibrary.org/obo/GAZ_00113948 -->

    <owl:NamedIndividual rdf:about="http://purl.obolibrary.org/obo/GAZ_00113948">
        <obo:RO_0001025 rdf:resource="http://purl.obolibrary.org/obo/GAZ_00032143"/>
        <obo:IAO_0000115>A commune of Tera Department.</obo:IAO_0000115>
        <oboInOwl:hasOBONamespace>GAZ</oboInOwl:hasOBONamespace>
        <oboInOwl:id>GAZ:00113948</oboInOwl:id>
        <rdfs:label>Communaute Urbaine de Tera</rdfs:label>
    </owl:NamedIndividual>
    


    <!-- http://purl.obolibrary.org/obo/GAZ_00113949 -->

    <owl:NamedIndividual rdf:about="http://purl.obolibrary.org/obo/GAZ_00113949">
        <obo:RO_0001025 rdf:resource="http://purl.obolibrary.org/obo/GAZ_00032143"/>
        <obo:IAO_0000115>A commune of Tera Department.</obo:IAO_0000115>
        <oboInOwl:hasOBONamespace>GAZ</oboInOwl:hasOBONamespace>
        <oboInOwl:id>GAZ:00113949</oboInOwl:id>
        <rdfs:label>Commune of Diagorou</rdfs:label>
    </owl:NamedIndividual>
    


    <!-- http://purl.obolibrary.org/obo/GAZ_00113950 -->

    <owl:NamedIndividual rdf:about="http://purl.obolibrary.org/obo/GAZ_00113950">
        <obo:RO_0001025 rdf:resource="http://purl.obolibrary.org/obo/GAZ_00032143"/>
        <obo:IAO_0000115>A commune of Tera Department.</obo:IAO_0000115>
        <oboInOwl:hasOBONamespace>GAZ</oboInOwl:hasOBONamespace>
        <oboInOwl:id>GAZ:00113950</oboInOwl:id>
        <rdfs:label>Commune of Kokorou</rdfs:label>
    </owl:NamedIndividual>
    


    <!-- http://purl.obolibrary.org/obo/GAZ_00113951 -->

    <owl:NamedIndividual rdf:about="http://purl.obolibrary.org/obo/GAZ_00113951">
        <obo:RO_0001025 rdf:resource="http://purl.obolibrary.org/obo/GAZ_00032143"/>
        <obo:IAO_0000115>A commune of Tera Department.</obo:IAO_0000115>
        <oboInOwl:hasOBONamespace>GAZ</oboInOwl:hasOBONamespace>
        <oboInOwl:id>GAZ:00113951</oboInOwl:id>
        <rdfs:label>Commune of Gorouol</rdfs:label>
    </owl:NamedIndividual>
    


    <!-- http://purl.obolibrary.org/obo/GAZ_00113952 -->

    <owl:NamedIndividual rdf:about="http://purl.obolibrary.org/obo/GAZ_00113952">
        <obo:RO_0001025 rdf:resource="http://purl.obolibrary.org/obo/GAZ_00032143"/>
        <obo:IAO_0000115>A commune of Tera Department.</obo:IAO_0000115>
        <oboInOwl:hasOBONamespace>GAZ</oboInOwl:hasOBONamespace>
        <oboInOwl:id>GAZ:00113952</oboInOwl:id>
        <rdfs:label>Commune of Dargol</rdfs:label>
    </owl:NamedIndividual>
    


    <!-- http://purl.obolibrary.org/obo/GAZ_00113953 -->

    <owl:NamedIndividual rdf:about="http://purl.obolibrary.org/obo/GAZ_00113953">
        <obo:RO_0001025 rdf:resource="http://purl.obolibrary.org/obo/GAZ_00032142"/>
        <obo:IAO_0000115>A commune of Say Department.</obo:IAO_0000115>
        <oboInOwl:hasOBONamespace>GAZ</oboInOwl:hasOBONamespace>
        <oboInOwl:id>GAZ:00113953</oboInOwl:id>
        <rdfs:label>Commune of Gueladjo</rdfs:label>
    </owl:NamedIndividual>
    


    <!-- http://purl.obolibrary.org/obo/GAZ_00113954 -->

    <owl:NamedIndividual rdf:about="http://purl.obolibrary.org/obo/GAZ_00113954">
        <obo:RO_0001025 rdf:resource="http://purl.obolibrary.org/obo/GAZ_00032142"/>
        <obo:IAO_0000115>A commune of Say Department.</obo:IAO_0000115>
        <oboInOwl:hasOBONamespace>GAZ</oboInOwl:hasOBONamespace>
        <oboInOwl:id>GAZ:00113954</oboInOwl:id>
        <rdfs:label>Commune of Tamou</rdfs:label>
    </owl:NamedIndividual>
    


    <!-- http://purl.obolibrary.org/obo/GAZ_00113955 -->

    <owl:NamedIndividual rdf:about="http://purl.obolibrary.org/obo/GAZ_00113955">
        <obo:RO_0001025 rdf:resource="http://purl.obolibrary.org/obo/GAZ_00032142"/>
        <obo:IAO_0000115>A commune of Say Department.</obo:IAO_0000115>
        <oboInOwl:hasOBONamespace>GAZ</oboInOwl:hasOBONamespace>
        <oboInOwl:id>GAZ:00113955</oboInOwl:id>
        <rdfs:label>Commune of Torodi</rdfs:label>
    </owl:NamedIndividual>
    


    <!-- http://purl.obolibrary.org/obo/GAZ_00113956 -->

    <owl:NamedIndividual rdf:about="http://purl.obolibrary.org/obo/GAZ_00113956">
        <obo:RO_0001025 rdf:resource="http://purl.obolibrary.org/obo/GAZ_00032142"/>
        <obo:IAO_0000115>A commune of Say Department.</obo:IAO_0000115>
        <oboInOwl:hasOBONamespace>GAZ</oboInOwl:hasOBONamespace>
        <oboInOwl:id>GAZ:00113956</oboInOwl:id>
        <rdfs:label>Communaute Urbaine de Say</rdfs:label>
    </owl:NamedIndividual>
    


    <!-- http://purl.obolibrary.org/obo/GAZ_00113957 -->

    <owl:NamedIndividual rdf:about="http://purl.obolibrary.org/obo/GAZ_00113957">
        <obo:RO_0001025 rdf:resource="http://purl.obolibrary.org/obo/GAZ_00032139"/>
        <obo:IAO_0000115>A commune in Ouallam Department.</obo:IAO_0000115>
        <oboInOwl:hasOBONamespace>GAZ</oboInOwl:hasOBONamespace>
        <oboInOwl:id>GAZ:00113957</oboInOwl:id>
        <rdfs:label>Communaute Urbaine de Ouallam</rdfs:label>
    </owl:NamedIndividual>
    


    <!-- http://purl.obolibrary.org/obo/GAZ_00113958 -->

    <owl:NamedIndividual rdf:about="http://purl.obolibrary.org/obo/GAZ_00113958">
        <obo:RO_0001025 rdf:resource="http://purl.obolibrary.org/obo/GAZ_00032141"/>
        <obo:IAO_0000115>A commune of Kollo Department.</obo:IAO_0000115>
        <oboInOwl:hasOBONamespace>GAZ</oboInOwl:hasOBONamespace>
        <oboInOwl:id>GAZ:00113958</oboInOwl:id>
        <rdfs:label>Commune of Hamdallay</rdfs:label>
    </owl:NamedIndividual>
    


    <!-- http://purl.obolibrary.org/obo/GAZ_00113959 -->

    <owl:NamedIndividual rdf:about="http://purl.obolibrary.org/obo/GAZ_00113959">
        <obo:RO_0001025 rdf:resource="http://purl.obolibrary.org/obo/GAZ_00032139"/>
        <obo:IAO_0000115>A commune in Ouallam Department.</obo:IAO_0000115>
        <oboInOwl:hasOBONamespace>GAZ</oboInOwl:hasOBONamespace>
        <oboInOwl:id>GAZ:00113959</oboInOwl:id>
        <rdfs:label>Commune of Dingazi</rdfs:label>
    </owl:NamedIndividual>
    


    <!-- http://purl.obolibrary.org/obo/GAZ_00113960 -->

    <owl:NamedIndividual rdf:about="http://purl.obolibrary.org/obo/GAZ_00113960">
        <obo:RO_0001025 rdf:resource="http://purl.obolibrary.org/obo/GAZ_00032139"/>
        <obo:IAO_0000115>A commune in Ouallam Department.</obo:IAO_0000115>
        <oboInOwl:hasOBONamespace>GAZ</oboInOwl:hasOBONamespace>
        <oboInOwl:id>GAZ:00113960</oboInOwl:id>
        <rdfs:label>Commune of Bani Bangou</rdfs:label>
    </owl:NamedIndividual>
    


    <!-- http://purl.obolibrary.org/obo/GAZ_00113961 -->

    <owl:NamedIndividual rdf:about="http://purl.obolibrary.org/obo/GAZ_00113961">
        <obo:RO_0001025 rdf:resource="http://purl.obolibrary.org/obo/GAZ_00032139"/>
        <obo:IAO_0000115>A commune in Ouallam Department.</obo:IAO_0000115>
        <oboInOwl:hasOBONamespace>GAZ</oboInOwl:hasOBONamespace>
        <oboInOwl:id>GAZ:00113961</oboInOwl:id>
        <rdfs:label>Commune of Tondikiwindi</rdfs:label>
    </owl:NamedIndividual>
    


    <!-- http://purl.obolibrary.org/obo/GAZ_00113962 -->

    <owl:NamedIndividual rdf:about="http://purl.obolibrary.org/obo/GAZ_00113962">
        <obo:RO_0001025 rdf:resource="http://purl.obolibrary.org/obo/GAZ_00032139"/>
        <obo:IAO_0000115>A commune in Ouallam Department.</obo:IAO_0000115>
        <oboInOwl:hasOBONamespace>GAZ</oboInOwl:hasOBONamespace>
        <oboInOwl:id>GAZ:00113962</oboInOwl:id>
        <rdfs:label>Commune of Simiri</rdfs:label>
    </owl:NamedIndividual>
    


    <!-- http://purl.obolibrary.org/obo/GAZ_00113963 -->

    <owl:NamedIndividual rdf:about="http://purl.obolibrary.org/obo/GAZ_00113963">
        <obo:RO_0001025 rdf:resource="http://purl.obolibrary.org/obo/GAZ_00032141"/>
        <obo:IAO_0000115>A commune of Kollo Department.</obo:IAO_0000115>
        <oboInOwl:hasOBONamespace>GAZ</oboInOwl:hasOBONamespace>
        <oboInOwl:id>GAZ:00113963</oboInOwl:id>
        <rdfs:label>Commune of Karma</rdfs:label>
    </owl:NamedIndividual>
    


    <!-- http://purl.obolibrary.org/obo/GAZ_00113964 -->

    <owl:NamedIndividual rdf:about="http://purl.obolibrary.org/obo/GAZ_00113964">
        <obo:RO_0001025 rdf:resource="http://purl.obolibrary.org/obo/GAZ_00032141"/>
        <obo:IAO_0000115>A commune of Kollo Department.</obo:IAO_0000115>
        <oboInOwl:hasOBONamespace>GAZ</oboInOwl:hasOBONamespace>
        <oboInOwl:id>GAZ:00113964</oboInOwl:id>
        <rdfs:label>Communaute Urbaine de Kollo</rdfs:label>
    </owl:NamedIndividual>
    


    <!-- http://purl.obolibrary.org/obo/GAZ_00113965 -->

    <owl:NamedIndividual rdf:about="http://purl.obolibrary.org/obo/GAZ_00113965">
        <obo:RO_0001025 rdf:resource="http://purl.obolibrary.org/obo/GAZ_00032141"/>
        <obo:IAO_0000115>A commune of Kollo Department.</obo:IAO_0000115>
        <oboInOwl:hasOBONamespace>GAZ</oboInOwl:hasOBONamespace>
        <oboInOwl:id>GAZ:00113965</oboInOwl:id>
        <rdfs:label>Commune of N&apos;Dounga</rdfs:label>
    </owl:NamedIndividual>
    


    <!-- http://purl.obolibrary.org/obo/GAZ_00113966 -->

    <owl:NamedIndividual rdf:about="http://purl.obolibrary.org/obo/GAZ_00113966">
        <obo:RO_0001025 rdf:resource="http://purl.obolibrary.org/obo/GAZ_00032141"/>
        <obo:IAO_0000115>A commune of Kollo Department.</obo:IAO_0000115>
        <oboInOwl:hasOBONamespace>GAZ</oboInOwl:hasOBONamespace>
        <oboInOwl:id>GAZ:00113966</oboInOwl:id>
        <rdfs:label>Commune of Namaro</rdfs:label>
    </owl:NamedIndividual>
    


    <!-- http://purl.obolibrary.org/obo/GAZ_00113967 -->

    <owl:NamedIndividual rdf:about="http://purl.obolibrary.org/obo/GAZ_00113967">
        <obo:RO_0001025 rdf:resource="http://purl.obolibrary.org/obo/GAZ_00032141"/>
        <obo:IAO_0000115>A commune of Kollo Department.</obo:IAO_0000115>
        <oboInOwl:hasOBONamespace>GAZ</oboInOwl:hasOBONamespace>
        <oboInOwl:id>GAZ:00113967</oboInOwl:id>
        <rdfs:label>Commune of Koure</rdfs:label>
    </owl:NamedIndividual>
    


    <!-- http://purl.obolibrary.org/obo/GAZ_00113968 -->

    <owl:NamedIndividual rdf:about="http://purl.obolibrary.org/obo/GAZ_00113968">
        <obo:RO_0001025 rdf:resource="http://purl.obolibrary.org/obo/GAZ_00032141"/>
        <obo:IAO_0000115>A commune of Kollo Department.</obo:IAO_0000115>
        <oboInOwl:hasOBONamespace>GAZ</oboInOwl:hasOBONamespace>
        <oboInOwl:id>GAZ:00113968</oboInOwl:id>
        <rdfs:label>Commune of Libore</rdfs:label>
    </owl:NamedIndividual>
    


    <!-- http://purl.obolibrary.org/obo/GAZ_00113969 -->

    <owl:NamedIndividual rdf:about="http://purl.obolibrary.org/obo/GAZ_00113969">
        <obo:RO_0001025 rdf:resource="http://purl.obolibrary.org/obo/GAZ_00032141"/>
        <obo:IAO_0000115>A commune of Kollo Department.</obo:IAO_0000115>
        <oboInOwl:hasOBONamespace>GAZ</oboInOwl:hasOBONamespace>
        <oboInOwl:id>GAZ:00113969</oboInOwl:id>
        <rdfs:label>Commune of Kirtachi</rdfs:label>
    </owl:NamedIndividual>
    


    <!-- http://purl.obolibrary.org/obo/GAZ_00113970 -->

    <owl:NamedIndividual rdf:about="http://purl.obolibrary.org/obo/GAZ_00113970">
        <obo:RO_0001025 rdf:resource="http://purl.obolibrary.org/obo/GAZ_00032141"/>
        <obo:IAO_0000115>A commune of Kollo Department.</obo:IAO_0000115>
        <oboInOwl:hasOBONamespace>GAZ</oboInOwl:hasOBONamespace>
        <oboInOwl:id>GAZ:00113970</oboInOwl:id>
        <rdfs:label>Commune of Fakara</rdfs:label>
    </owl:NamedIndividual>
    


    <!-- http://purl.obolibrary.org/obo/GAZ_00113971 -->

    <owl:NamedIndividual rdf:about="http://purl.obolibrary.org/obo/GAZ_00113971">
        <obo:RO_0001025 rdf:resource="http://purl.obolibrary.org/obo/GAZ_00032141"/>
        <obo:IAO_0000115>A commune of Kollo Department.</obo:IAO_0000115>
        <oboInOwl:hasOBONamespace>GAZ</oboInOwl:hasOBONamespace>
        <oboInOwl:id>GAZ:00113971</oboInOwl:id>
        <rdfs:label>Commune of Lamorde</rdfs:label>
    </owl:NamedIndividual>
    


    <!-- http://purl.obolibrary.org/obo/GAZ_00113972 -->

    <owl:NamedIndividual rdf:about="http://purl.obolibrary.org/obo/GAZ_00113972">
        <obo:RO_0001025 rdf:resource="http://purl.obolibrary.org/obo/GAZ_00032144"/>
        <obo:IAO_0000115>A commune of Filingue Department.</obo:IAO_0000115>
        <oboInOwl:hasOBONamespace>GAZ</oboInOwl:hasOBONamespace>
        <oboInOwl:id>GAZ:00113972</oboInOwl:id>
        <rdfs:label>Commune of Tabala</rdfs:label>
    </owl:NamedIndividual>
    


    <!-- http://purl.obolibrary.org/obo/GAZ_00113973 -->

    <owl:NamedIndividual rdf:about="http://purl.obolibrary.org/obo/GAZ_00113973">
        <obo:RO_0001025 rdf:resource="http://purl.obolibrary.org/obo/GAZ_00032144"/>
        <obo:IAO_0000115>A commune of Filingue Department.</obo:IAO_0000115>
        <oboInOwl:hasOBONamespace>GAZ</oboInOwl:hasOBONamespace>
        <oboInOwl:id>GAZ:00113973</oboInOwl:id>
        <rdfs:label>Commune of Konfey</rdfs:label>
    </owl:NamedIndividual>
    


    <!-- http://purl.obolibrary.org/obo/GAZ_00113974 -->

    <owl:NamedIndividual rdf:about="http://purl.obolibrary.org/obo/GAZ_00113974">
        <obo:RO_0001025 rdf:resource="http://purl.obolibrary.org/obo/GAZ_00032144"/>
        <obo:IAO_0000115>A commune of Filingue Department.</obo:IAO_0000115>
        <oboInOwl:hasOBONamespace>GAZ</oboInOwl:hasOBONamespace>
        <oboInOwl:id>GAZ:00113974</oboInOwl:id>
        <rdfs:label>Commune of Tondikandia</rdfs:label>
    </owl:NamedIndividual>
    


    <!-- http://purl.obolibrary.org/obo/GAZ_00113975 -->

    <owl:NamedIndividual rdf:about="http://purl.obolibrary.org/obo/GAZ_00113975">
        <obo:RO_0001025 rdf:resource="http://purl.obolibrary.org/obo/GAZ_00032144"/>
        <obo:IAO_0000115>A commune of Filingue Department.</obo:IAO_0000115>
        <oboInOwl:hasOBONamespace>GAZ</oboInOwl:hasOBONamespace>
        <oboInOwl:id>GAZ:00113975</oboInOwl:id>
        <rdfs:label>Commune of Bonkoukou</rdfs:label>
    </owl:NamedIndividual>
    


    <!-- http://purl.obolibrary.org/obo/GAZ_00113976 -->

    <owl:NamedIndividual rdf:about="http://purl.obolibrary.org/obo/GAZ_00113976">
        <obo:RO_0001025 rdf:resource="http://purl.obolibrary.org/obo/GAZ_00032144"/>
        <obo:IAO_0000115>A commune of Filingue Department.</obo:IAO_0000115>
        <oboInOwl:hasOBONamespace>GAZ</oboInOwl:hasOBONamespace>
        <oboInOwl:id>GAZ:00113976</oboInOwl:id>
        <rdfs:label>Communaute Urbaine de Filingue</rdfs:label>
    </owl:NamedIndividual>
    


    <!-- http://purl.obolibrary.org/obo/GAZ_00113977 -->

    <owl:NamedIndividual rdf:about="http://purl.obolibrary.org/obo/GAZ_00113977">
        <obo:RO_0001025 rdf:resource="http://purl.obolibrary.org/obo/GAZ_00000826"/>
        <obo:IAO_0000115>A department of the Tahoua Region in Niger. Its capital lies at the city of Abalak.</obo:IAO_0000115>
        <oboInOwl:hasOBONamespace>GAZ</oboInOwl:hasOBONamespace>
        <oboInOwl:id>GAZ:00113977</oboInOwl:id>
        <rdfs:label>Abalak Department</rdfs:label>
    </owl:NamedIndividual>
    


    <!-- http://purl.obolibrary.org/obo/GAZ_00113978 -->

    <owl:NamedIndividual rdf:about="http://purl.obolibrary.org/obo/GAZ_00113978">
        <obo:RO_0001025 rdf:resource="http://purl.obolibrary.org/obo/GAZ_00032138"/>
        <obo:IAO_0000115>A Communaute Urbaine.</obo:IAO_0000115>
        <oboInOwl:hasOBONamespace>GAZ</oboInOwl:hasOBONamespace>
        <oboInOwl:id>GAZ:00113978</oboInOwl:id>
        <rdfs:label>Communaute Urbaine de Tchin Tabaradine</rdfs:label>
    </owl:NamedIndividual>
    


    <!-- http://purl.obolibrary.org/obo/GAZ_00113979 -->

    <owl:NamedIndividual rdf:about="http://purl.obolibrary.org/obo/GAZ_00113979">
        <obo:RO_0001025 rdf:resource="http://purl.obolibrary.org/obo/GAZ_00032135"/>
        <obo:IAO_0000115>A Communaute Urbaine.</obo:IAO_0000115>
        <oboInOwl:hasOBONamespace>GAZ</oboInOwl:hasOBONamespace>
        <oboInOwl:id>GAZ:00113979</oboInOwl:id>
        <rdfs:label>Communaute Urbaine de Madaoua</rdfs:label>
    </owl:NamedIndividual>
    


    <!-- http://purl.obolibrary.org/obo/GAZ_00113980 -->

    <owl:NamedIndividual rdf:about="http://purl.obolibrary.org/obo/GAZ_00113980">
        <obo:RO_0001025 rdf:resource="http://purl.obolibrary.org/obo/GAZ_00032137"/>
        <obo:IAO_0000115>A commune of Tahoua Department.</obo:IAO_0000115>
        <oboInOwl:hasOBONamespace>GAZ</oboInOwl:hasOBONamespace>
        <oboInOwl:id>GAZ:00113980</oboInOwl:id>
        <rdfs:label>Commune of Bambay</rdfs:label>
    </owl:NamedIndividual>
    


    <!-- http://purl.obolibrary.org/obo/GAZ_00113981 -->

    <owl:NamedIndividual rdf:about="http://purl.obolibrary.org/obo/GAZ_00113981">
        <obo:RO_0001025 rdf:resource="http://purl.obolibrary.org/obo/GAZ_00032137"/>
        <obo:IAO_0000115>A Communaute Urbaine of Tahoua Department.</obo:IAO_0000115>
        <oboInOwl:hasOBONamespace>GAZ</oboInOwl:hasOBONamespace>
        <oboInOwl:id>GAZ:00113981</oboInOwl:id>
        <rdfs:label>Communaute Urbaine de Tahoua</rdfs:label>
    </owl:NamedIndividual>
    


    <!-- http://purl.obolibrary.org/obo/GAZ_00113982 -->

    <owl:NamedIndividual rdf:about="http://purl.obolibrary.org/obo/GAZ_00113982">
        <obo:RO_0001025 rdf:resource="http://purl.obolibrary.org/obo/GAZ_00032137"/>
        <obo:IAO_0000115>A commune of Tahoua Department.</obo:IAO_0000115>
        <oboInOwl:hasOBONamespace>GAZ</oboInOwl:hasOBONamespace>
        <oboInOwl:id>GAZ:00113982</oboInOwl:id>
        <rdfs:label>Commune of Kalkou</rdfs:label>
    </owl:NamedIndividual>
    


    <!-- http://purl.obolibrary.org/obo/GAZ_00113983 -->

    <owl:NamedIndividual rdf:about="http://purl.obolibrary.org/obo/GAZ_00113983">
        <obo:RO_0001025 rdf:resource="http://purl.obolibrary.org/obo/GAZ_00032134"/>
        <obo:IAO_0000115>A Communaute Urbaine.</obo:IAO_0000115>
        <oboInOwl:hasOBONamespace>GAZ</oboInOwl:hasOBONamespace>
        <oboInOwl:id>GAZ:00113983</oboInOwl:id>
        <rdfs:label>Communaute Urbaine de llela/Tajae</rdfs:label>
    </owl:NamedIndividual>
    


    <!-- http://purl.obolibrary.org/obo/GAZ_00113984 -->

    <owl:NamedIndividual rdf:about="http://purl.obolibrary.org/obo/GAZ_00113984">
        <obo:RO_0001025 rdf:resource="http://purl.obolibrary.org/obo/GAZ_00000826"/>
        <obo:IAO_0000115>A department of the Tahoua Region in Niger. Its capital lies at the city of Birni N&apos;konni.</obo:IAO_0000115>
        <oboInOwl:hasOBONamespace>GAZ</oboInOwl:hasOBONamespace>
        <oboInOwl:id>GAZ:00113984</oboInOwl:id>
        <rdfs:label>Birni N&apos;konni Department</rdfs:label>
    </owl:NamedIndividual>
    


    <!-- http://purl.obolibrary.org/obo/GAZ_00113985 -->

    <owl:NamedIndividual rdf:about="http://purl.obolibrary.org/obo/GAZ_00113985">
        <obo:RO_0001025 rdf:resource="http://purl.obolibrary.org/obo/GAZ_00113984"/>
        <obo:IAO_0000115>A Communaute Urbaine.</obo:IAO_0000115>
        <oboInOwl:hasOBONamespace>GAZ</oboInOwl:hasOBONamespace>
        <oboInOwl:id>GAZ:00113985</oboInOwl:id>
        <rdfs:label>Communaute Urbaine de Birni N&apos;konni</rdfs:label>
    </owl:NamedIndividual>
    


    <!-- http://purl.obolibrary.org/obo/GAZ_00113986 -->

    <owl:NamedIndividual rdf:about="http://purl.obolibrary.org/obo/GAZ_00113986">
        <obo:RO_0001025 rdf:resource="http://purl.obolibrary.org/obo/GAZ_00113977"/>
        <obo:IAO_0000115>A Communaute Urbaine.</obo:IAO_0000115>
        <oboInOwl:hasOBONamespace>GAZ</oboInOwl:hasOBONamespace>
        <oboInOwl:id>GAZ:00113986</oboInOwl:id>
        <rdfs:label>Communaute Urbaine de Abalak</rdfs:label>
    </owl:NamedIndividual>
    


    <!-- http://purl.obolibrary.org/obo/GAZ_00113987 -->

    <owl:NamedIndividual rdf:about="http://purl.obolibrary.org/obo/GAZ_00113987">
        <obo:RO_0001025 rdf:resource="http://purl.obolibrary.org/obo/GAZ_00032132"/>
        <obo:IAO_0000115>A Communaute Urbaine.</obo:IAO_0000115>
        <oboInOwl:hasOBONamespace>GAZ</oboInOwl:hasOBONamespace>
        <oboInOwl:id>GAZ:00113987</oboInOwl:id>
        <rdfs:label>Communaute Urbaine de Bouza</rdfs:label>
    </owl:NamedIndividual>
    


    <!-- http://purl.obolibrary.org/obo/GAZ_00113988 -->

    <owl:NamedIndividual rdf:about="http://purl.obolibrary.org/obo/GAZ_00113988">
        <obo:RO_0001025 rdf:resource="http://purl.obolibrary.org/obo/GAZ_00113981"/>
        <obo:IAO_0000115>A commune of the Communaute Urbaine de Tahoua.</obo:IAO_0000115>
        <oboInOwl:hasOBONamespace>GAZ</oboInOwl:hasOBONamespace>
        <oboInOwl:id>GAZ:00113988</oboInOwl:id>
        <rdfs:label>Commune of Tahoua II</rdfs:label>
    </owl:NamedIndividual>
    


    <!-- http://purl.obolibrary.org/obo/GAZ_00113989 -->

    <owl:NamedIndividual rdf:about="http://purl.obolibrary.org/obo/GAZ_00113989">
        <obo:RO_0001025 rdf:resource="http://purl.obolibrary.org/obo/GAZ_00113981"/>
        <obo:IAO_0000115>A commune of the Communaute Urbaine de Tahoua.</obo:IAO_0000115>
        <oboInOwl:hasOBONamespace>GAZ</oboInOwl:hasOBONamespace>
        <oboInOwl:id>GAZ:00113989</oboInOwl:id>
        <rdfs:label>Commune of Tahoua I</rdfs:label>
    </owl:NamedIndividual>
    


    <!-- http://purl.obolibrary.org/obo/GAZ_00113990 -->

    <owl:NamedIndividual rdf:about="http://purl.obolibrary.org/obo/GAZ_00113990">
        <obo:RO_0001025 rdf:resource="http://purl.obolibrary.org/obo/GAZ_00032137"/>
        <obo:IAO_0000115>A commune of Tahoua Department.</obo:IAO_0000115>
        <oboInOwl:hasOBONamespace>GAZ</oboInOwl:hasOBONamespace>
        <oboInOwl:id>GAZ:00113990</oboInOwl:id>
        <rdfs:label>Commune of Affala</rdfs:label>
    </owl:NamedIndividual>
    


    <!-- http://purl.obolibrary.org/obo/GAZ_00113991 -->

    <owl:NamedIndividual rdf:about="http://purl.obolibrary.org/obo/GAZ_00113991">
        <obo:RO_0001025 rdf:resource="http://purl.obolibrary.org/obo/GAZ_00032137"/>
        <obo:IAO_0000115>A commune of Tahoua Department.</obo:IAO_0000115>
        <oboInOwl:hasOBONamespace>GAZ</oboInOwl:hasOBONamespace>
        <oboInOwl:id>GAZ:00113991</oboInOwl:id>
        <rdfs:label>Commune of Barmo</rdfs:label>
    </owl:NamedIndividual>
    


    <!-- http://purl.obolibrary.org/obo/GAZ_00113992 -->

    <owl:NamedIndividual rdf:about="http://purl.obolibrary.org/obo/GAZ_00113992">
        <obo:RO_0001025 rdf:resource="http://purl.obolibrary.org/obo/GAZ_00032133"/>
        <oboInOwl:hasOBONamespace>GAZ</oboInOwl:hasOBONamespace>
        <oboInOwl:id>GAZ:00113992</oboInOwl:id>
        <rdfs:label>Communaute Urbaine de Keita</rdfs:label>
    </owl:NamedIndividual>
    


    <!-- http://purl.obolibrary.org/obo/GAZ_00113993 -->

    <owl:NamedIndividual rdf:about="http://purl.obolibrary.org/obo/GAZ_00113993">
        <obo:RO_0001025 rdf:resource="http://purl.obolibrary.org/obo/GAZ_00032120"/>
        <obo:IAO_0000115>A Communaute Urbaine.</obo:IAO_0000115>
        <oboInOwl:hasOBONamespace>GAZ</oboInOwl:hasOBONamespace>
        <oboInOwl:id>GAZ:00113993</oboInOwl:id>
        <rdfs:label>Communaute Urbaine de Dosso</rdfs:label>
    </owl:NamedIndividual>
    


    <!-- http://purl.obolibrary.org/obo/GAZ_00113994 -->

    <owl:NamedIndividual rdf:about="http://purl.obolibrary.org/obo/GAZ_00113994">
        <obo:RO_0001025 rdf:resource="http://purl.obolibrary.org/obo/GAZ_00032122"/>
        <obo:IAO_0000115>A commune.</obo:IAO_0000115>
        <oboInOwl:hasOBONamespace>GAZ</oboInOwl:hasOBONamespace>
        <oboInOwl:id>GAZ:00113994</oboInOwl:id>
        <rdfs:label>Commune of Harikanassou</rdfs:label>
    </owl:NamedIndividual>
    


    <!-- http://purl.obolibrary.org/obo/GAZ_00113995 -->

    <owl:NamedIndividual rdf:about="http://purl.obolibrary.org/obo/GAZ_00113995">
        <obo:RO_0001025 rdf:resource="http://purl.obolibrary.org/obo/GAZ_00032122"/>
        <obo:IAO_0000115>A Communaute Urbaine.</obo:IAO_0000115>
        <oboInOwl:hasOBONamespace>GAZ</oboInOwl:hasOBONamespace>
        <oboInOwl:id>GAZ:00113995</oboInOwl:id>
        <rdfs:label>Communaute Urbaine de Birni N&apos;Gaoure</rdfs:label>
    </owl:NamedIndividual>
    


    <!-- http://purl.obolibrary.org/obo/GAZ_00113996 -->

    <owl:NamedIndividual rdf:about="http://purl.obolibrary.org/obo/GAZ_00113996">
        <obo:RO_0001025 rdf:resource="http://purl.obolibrary.org/obo/GAZ_00032122"/>
        <obo:IAO_0000115>A commune.</obo:IAO_0000115>
        <oboInOwl:hasOBONamespace>GAZ</oboInOwl:hasOBONamespace>
        <oboInOwl:id>GAZ:00113996</oboInOwl:id>
        <rdfs:label>Commune of Koygolo</rdfs:label>
    </owl:NamedIndividual>
    


    <!-- http://purl.obolibrary.org/obo/GAZ_00113997 -->

    <owl:NamedIndividual rdf:about="http://purl.obolibrary.org/obo/GAZ_00113997">
        <obo:RO_0001025 rdf:resource="http://purl.obolibrary.org/obo/GAZ_00032122"/>
        <obo:IAO_0000115>A commune ?</obo:IAO_0000115>
        <oboInOwl:hasOBONamespace>GAZ</oboInOwl:hasOBONamespace>
        <oboInOwl:id>GAZ:00113997</oboInOwl:id>
        <rdfs:label>Commune of Boboye</rdfs:label>
    </owl:NamedIndividual>
    


    <!-- http://purl.obolibrary.org/obo/GAZ_00113998 -->

    <owl:NamedIndividual rdf:about="http://purl.obolibrary.org/obo/GAZ_00113998">
        <obo:RO_0001025 rdf:resource="http://purl.obolibrary.org/obo/GAZ_00032124"/>
        <obo:IAO_0000115>A commune.</obo:IAO_0000115>
        <oboInOwl:hasOBONamespace>GAZ</oboInOwl:hasOBONamespace>
        <oboInOwl:id>GAZ:00113998</oboInOwl:id>
        <rdfs:label>Commune of Takassaba</rdfs:label>
    </owl:NamedIndividual>
    


    <!-- http://purl.obolibrary.org/obo/GAZ_00113999 -->

    <owl:NamedIndividual rdf:about="http://purl.obolibrary.org/obo/GAZ_00113999">
        <obo:RO_0001025 rdf:resource="http://purl.obolibrary.org/obo/GAZ_00032124"/>
        <obo:IAO_0000115>A Communaute Urbaine.</obo:IAO_0000115>
        <oboInOwl:hasOBONamespace>GAZ</oboInOwl:hasOBONamespace>
        <oboInOwl:id>GAZ:00113999</oboInOwl:id>
        <rdfs:label>Communaute Urbaine de Dogondoutchi</rdfs:label>
    </owl:NamedIndividual>
    


    <!-- http://purl.obolibrary.org/obo/GAZ_00114000 -->

    <owl:NamedIndividual rdf:about="http://purl.obolibrary.org/obo/GAZ_00114000">
        <obo:RO_0001025 rdf:resource="http://purl.obolibrary.org/obo/GAZ_00032124"/>
        <obo:IAO_0000115>A commune.</obo:IAO_0000115>
        <oboInOwl:hasOBONamespace>GAZ</oboInOwl:hasOBONamespace>
        <oboInOwl:id>GAZ:00114000</oboInOwl:id>
        <rdfs:label>Commune of Tibir</rdfs:label>
    </owl:NamedIndividual>
    


    <!-- http://purl.obolibrary.org/obo/GAZ_00114001 -->

    <owl:NamedIndividual rdf:about="http://purl.obolibrary.org/obo/GAZ_00114001">
        <obo:RO_0001025 rdf:resource="http://purl.obolibrary.org/obo/GAZ_00032123"/>
        <obo:IAO_0000115>A Communaute Urbaine.</obo:IAO_0000115>
        <oboInOwl:hasOBONamespace>GAZ</oboInOwl:hasOBONamespace>
        <oboInOwl:id>GAZ:00114001</oboInOwl:id>
        <rdfs:label>Communaute Urbaine de Gaya</rdfs:label>
    </owl:NamedIndividual>
    


    <!-- http://purl.obolibrary.org/obo/GAZ_00114002 -->

    <owl:NamedIndividual rdf:about="http://purl.obolibrary.org/obo/GAZ_00114002">
        <obo:RO_0001025 rdf:resource="http://purl.obolibrary.org/obo/GAZ_00032123"/>
        <obo:IAO_0000115>A commune.</obo:IAO_0000115>
        <oboInOwl:hasOBONamespace>GAZ</oboInOwl:hasOBONamespace>
        <oboInOwl:id>GAZ:00114002</oboInOwl:id>
        <rdfs:label>Commune of Karakara</rdfs:label>
    </owl:NamedIndividual>
    


    <!-- http://purl.obolibrary.org/obo/GAZ_00114003 -->

    <owl:NamedIndividual rdf:about="http://purl.obolibrary.org/obo/GAZ_00114003">
        <obo:RO_0001025 rdf:resource="http://purl.obolibrary.org/obo/GAZ_00032123"/>
        <obo:IAO_0000115>A commune.</obo:IAO_0000115>
        <oboInOwl:hasOBONamespace>GAZ</oboInOwl:hasOBONamespace>
        <oboInOwl:id>GAZ:00114003</oboInOwl:id>
        <rdfs:label>Commune of Zabori</rdfs:label>
    </owl:NamedIndividual>
    


    <!-- http://purl.obolibrary.org/obo/GAZ_00114004 -->

    <owl:NamedIndividual rdf:about="http://purl.obolibrary.org/obo/GAZ_00114004">
        <obo:RO_0001025 rdf:resource="http://purl.obolibrary.org/obo/GAZ_00032123"/>
        <obo:IAO_0000115>A commune.</obo:IAO_0000115>
        <oboInOwl:hasOBONamespace>GAZ</oboInOwl:hasOBONamespace>
        <oboInOwl:id>GAZ:00114004</oboInOwl:id>
        <rdfs:label>Commune of Dioundiou</rdfs:label>
    </owl:NamedIndividual>
    


    <!-- http://purl.obolibrary.org/obo/GAZ_00114005 -->

    <owl:NamedIndividual rdf:about="http://purl.obolibrary.org/obo/GAZ_00114005">
        <obo:RO_0001025 rdf:resource="http://purl.obolibrary.org/obo/GAZ_00032123"/>
        <obo:IAO_0000115>A commune.</obo:IAO_0000115>
        <oboInOwl:hasOBONamespace>GAZ</oboInOwl:hasOBONamespace>
        <oboInOwl:id>GAZ:00114005</oboInOwl:id>
        <rdfs:label>Commune of Yelou</rdfs:label>
    </owl:NamedIndividual>
    


    <!-- http://purl.obolibrary.org/obo/GAZ_00114006 -->

    <owl:NamedIndividual rdf:about="http://purl.obolibrary.org/obo/GAZ_00114006">
        <obo:RO_0001025 rdf:resource="http://purl.obolibrary.org/obo/GAZ_00032123"/>
        <obo:IAO_0000115>A commune.</obo:IAO_0000115>
        <oboInOwl:hasOBONamespace>GAZ</oboInOwl:hasOBONamespace>
        <oboInOwl:id>GAZ:00114006</oboInOwl:id>
        <rdfs:label>Commune of Bana</rdfs:label>
    </owl:NamedIndividual>
    


    <!-- http://purl.obolibrary.org/obo/GAZ_00114007 -->

    <owl:NamedIndividual rdf:about="http://purl.obolibrary.org/obo/GAZ_00114007">
        <obo:RO_0001025 rdf:resource="http://purl.obolibrary.org/obo/GAZ_00032121"/>
        <obo:IAO_0000115>A commune.</obo:IAO_0000115>
        <oboInOwl:hasOBONamespace>GAZ</oboInOwl:hasOBONamespace>
        <oboInOwl:id>GAZ:00114007</oboInOwl:id>
        <rdfs:label>Commune of Goubey</rdfs:label>
    </owl:NamedIndividual>
    


    <!-- http://purl.obolibrary.org/obo/GAZ_00114008 -->

    <owl:NamedIndividual rdf:about="http://purl.obolibrary.org/obo/GAZ_00114008">
        <obo:RO_0001025 rdf:resource="http://purl.obolibrary.org/obo/GAZ_00032121"/>
        <obo:IAO_0000115>A Communaute Urbaine.</obo:IAO_0000115>
        <oboInOwl:hasOBONamespace>GAZ</oboInOwl:hasOBONamespace>
        <oboInOwl:id>GAZ:00114008</oboInOwl:id>
        <rdfs:label>Communaute Urbaine de Loga</rdfs:label>
    </owl:NamedIndividual>
    


    <!-- http://purl.obolibrary.org/obo/GAZ_00114009 -->

    <owl:NamedIndividual rdf:about="http://purl.obolibrary.org/obo/GAZ_00114009">
        <obo:RO_0001025 rdf:resource="http://purl.obolibrary.org/obo/GAZ_00032121"/>
        <obo:IAO_0000115>A commune.</obo:IAO_0000115>
        <oboInOwl:hasOBONamespace>GAZ</oboInOwl:hasOBONamespace>
        <oboInOwl:id>GAZ:00114009</oboInOwl:id>
        <rdfs:label>Commune of Sokorbe</rdfs:label>
    </owl:NamedIndividual>
    


    <!-- http://purl.obolibrary.org/obo/GAZ_00114010 -->

    <owl:NamedIndividual rdf:about="http://purl.obolibrary.org/obo/GAZ_00114010">
        <obo:RO_0001025 rdf:resource="http://purl.obolibrary.org/obo/GAZ_00032121"/>
        <obo:IAO_0000115>A commune.</obo:IAO_0000115>
        <oboInOwl:hasOBONamespace>GAZ</oboInOwl:hasOBONamespace>
        <oboInOwl:id>GAZ:00114010</oboInOwl:id>
        <rdfs:label>Commune of Falwal</rdfs:label>
    </owl:NamedIndividual>
    


    <!-- http://purl.obolibrary.org/obo/GAZ_00114011 -->

    <owl:NamedIndividual rdf:about="http://purl.obolibrary.org/obo/GAZ_00114011">
        <obo:RO_0001025 rdf:resource="http://purl.obolibrary.org/obo/GAZ_00000825"/>
        <oboInOwl:hasOBONamespace>GAZ</oboInOwl:hasOBONamespace>
        <oboInOwl:id>GAZ:00114011</oboInOwl:id>
        <rdfs:label>Communaute Urbaine de Maradi</rdfs:label>
    </owl:NamedIndividual>
    


    <!-- http://purl.obolibrary.org/obo/GAZ_00114012 -->

    <owl:NamedIndividual rdf:about="http://purl.obolibrary.org/obo/GAZ_00114012">
        <obo:RO_0001025 rdf:resource="http://purl.obolibrary.org/obo/GAZ_00114011"/>
        <oboInOwl:hasOBONamespace>GAZ</oboInOwl:hasOBONamespace>
        <oboInOwl:id>GAZ:00114012</oboInOwl:id>
        <rdfs:label>Commune of Maradi III</rdfs:label>
    </owl:NamedIndividual>
    


    <!-- http://purl.obolibrary.org/obo/GAZ_00114013 -->

    <owl:NamedIndividual rdf:about="http://purl.obolibrary.org/obo/GAZ_00114013">
        <obo:RO_0001025 rdf:resource="http://purl.obolibrary.org/obo/GAZ_00114011"/>
        <oboInOwl:hasOBONamespace>GAZ</oboInOwl:hasOBONamespace>
        <oboInOwl:id>GAZ:00114013</oboInOwl:id>
        <rdfs:label>Commune of Maradi II</rdfs:label>
    </owl:NamedIndividual>
    


    <!-- http://purl.obolibrary.org/obo/GAZ_00114014 -->

    <owl:NamedIndividual rdf:about="http://purl.obolibrary.org/obo/GAZ_00114014">
        <obo:RO_0001025 rdf:resource="http://purl.obolibrary.org/obo/GAZ_00114011"/>
        <oboInOwl:hasOBONamespace>GAZ</oboInOwl:hasOBONamespace>
        <oboInOwl:id>GAZ:00114014</oboInOwl:id>
        <rdfs:label>Commune of Maradi I</rdfs:label>
    </owl:NamedIndividual>
    


    <!-- http://purl.obolibrary.org/obo/GAZ_00114015 -->

    <owl:NamedIndividual rdf:about="http://purl.obolibrary.org/obo/GAZ_00114015">
        <obo:RO_0001025 rdf:resource="http://purl.obolibrary.org/obo/GAZ_00000822"/>
        <obo:IAO_0000115>A department of the Agadez Region in Niger. Its capital lies at the city of Arlit.</obo:IAO_0000115>
        <oboInOwl:hasOBONamespace>GAZ</oboInOwl:hasOBONamespace>
        <oboInOwl:id>GAZ:00114015</oboInOwl:id>
        <rdfs:label>Arlit Department</rdfs:label>
    </owl:NamedIndividual>
    


    <!-- http://purl.obolibrary.org/obo/GAZ_00114016 -->

    <owl:NamedIndividual rdf:about="http://purl.obolibrary.org/obo/GAZ_00114016">
        <obo:RO_0001025 rdf:resource="http://purl.obolibrary.org/obo/GAZ_00114015"/>
        <obo:IAO_0000115>A commune of Arlit Department.</obo:IAO_0000115>
        <oboInOwl:hasOBONamespace>GAZ</oboInOwl:hasOBONamespace>
        <oboInOwl:id>GAZ:00114016</oboInOwl:id>
        <rdfs:label>Commune of Inignaouei</rdfs:label>
    </owl:NamedIndividual>
    


    <!-- http://purl.obolibrary.org/obo/GAZ_00114017 -->

    <owl:NamedIndividual rdf:about="http://purl.obolibrary.org/obo/GAZ_00114017">
        <obo:RO_0001025 rdf:resource="http://purl.obolibrary.org/obo/GAZ_00114015"/>
        <obo:IAO_0000115>A commune of Arlit Department.</obo:IAO_0000115>
        <oboInOwl:hasOBONamespace>GAZ</oboInOwl:hasOBONamespace>
        <oboInOwl:id>GAZ:00114017</oboInOwl:id>
        <rdfs:label>Commune of Oubandawaki Makiani</rdfs:label>
    </owl:NamedIndividual>
    


    <!-- http://purl.obolibrary.org/obo/GAZ_00114018 -->

    <owl:NamedIndividual rdf:about="http://purl.obolibrary.org/obo/GAZ_00114018">
        <obo:RO_0001025 rdf:resource="http://purl.obolibrary.org/obo/GAZ_00114015"/>
        <obo:IAO_0000115>A commune of Arlit Department.</obo:IAO_0000115>
        <oboInOwl:hasOBONamespace>GAZ</oboInOwl:hasOBONamespace>
        <oboInOwl:id>GAZ:00114018</oboInOwl:id>
        <rdfs:label>Commune of Imourarene</rdfs:label>
    </owl:NamedIndividual>
    


    <!-- http://purl.obolibrary.org/obo/GAZ_00114019 -->

    <owl:NamedIndividual rdf:about="http://purl.obolibrary.org/obo/GAZ_00114019">
        <obo:RO_0001025 rdf:resource="http://purl.obolibrary.org/obo/GAZ_00114015"/>
        <obo:IAO_0000115>A commune of Arlit Department.</obo:IAO_0000115>
        <oboInOwl:hasOBONamespace>GAZ</oboInOwl:hasOBONamespace>
        <oboInOwl:id>GAZ:00114019</oboInOwl:id>
        <rdfs:label>Commune of Taggafadi</rdfs:label>
    </owl:NamedIndividual>
    


    <!-- http://purl.obolibrary.org/obo/GAZ_00114020 -->

    <owl:NamedIndividual rdf:about="http://purl.obolibrary.org/obo/GAZ_00114020">
        <obo:RO_0001025 rdf:resource="http://purl.obolibrary.org/obo/GAZ_00114015"/>
        <obo:IAO_0000115>A commune of Arlit Department.</obo:IAO_0000115>
        <oboInOwl:hasOBONamespace>GAZ</oboInOwl:hasOBONamespace>
        <oboInOwl:id>GAZ:00114020</oboInOwl:id>
        <rdfs:label>Commune of Elok</rdfs:label>
    </owl:NamedIndividual>
    


    <!-- http://purl.obolibrary.org/obo/GAZ_00114021 -->

    <owl:NamedIndividual rdf:about="http://purl.obolibrary.org/obo/GAZ_00114021">
        <obo:RO_0001025 rdf:resource="http://purl.obolibrary.org/obo/GAZ_00114015"/>
        <obo:IAO_0000115>A commune of Arlit Department.</obo:IAO_0000115>
        <oboInOwl:hasOBONamespace>GAZ</oboInOwl:hasOBONamespace>
        <oboInOwl:id>GAZ:00114021</oboInOwl:id>
        <rdfs:label>Commune of Tarhmert</rdfs:label>
    </owl:NamedIndividual>
    


    <!-- http://purl.obolibrary.org/obo/GAZ_00114022 -->

    <owl:NamedIndividual rdf:about="http://purl.obolibrary.org/obo/GAZ_00114022">
        <obo:RO_0001025 rdf:resource="http://purl.obolibrary.org/obo/GAZ_00114015"/>
        <obo:IAO_0000115>A Communaute Urbaine of Arlit Department.</obo:IAO_0000115>
        <oboInOwl:hasOBONamespace>GAZ</oboInOwl:hasOBONamespace>
        <oboInOwl:id>GAZ:00114022</oboInOwl:id>
        <rdfs:label>Communaute Urbaine de Arlit</rdfs:label>
    </owl:NamedIndividual>
    


    <!-- http://purl.obolibrary.org/obo/GAZ_00114023 -->

    <owl:NamedIndividual rdf:about="http://purl.obolibrary.org/obo/GAZ_00114023">
        <obo:RO_0001025 rdf:resource="http://purl.obolibrary.org/obo/GAZ_00114015"/>
        <obo:IAO_0000115>A commune of Arlit Department.</obo:IAO_0000115>
        <oboInOwl:hasOBONamespace>GAZ</oboInOwl:hasOBONamespace>
        <oboInOwl:id>GAZ:00114023</oboInOwl:id>
        <rdfs:label>Commune of Teouat</rdfs:label>
    </owl:NamedIndividual>
    


    <!-- http://purl.obolibrary.org/obo/GAZ_00114024 -->

    <owl:NamedIndividual rdf:about="http://purl.obolibrary.org/obo/GAZ_00114024">
        <obo:RO_0001025 rdf:resource="http://purl.obolibrary.org/obo/GAZ_00114015"/>
        <obo:IAO_0000115>A commune of Arlit Department.</obo:IAO_0000115>
        <oboInOwl:hasOBONamespace>GAZ</oboInOwl:hasOBONamespace>
        <oboInOwl:id>GAZ:00114024</oboInOwl:id>
        <rdfs:label>Commune of Gougaram</rdfs:label>
    </owl:NamedIndividual>
    


    <!-- http://purl.obolibrary.org/obo/GAZ_00114025 -->

    <owl:NamedIndividual rdf:about="http://purl.obolibrary.org/obo/GAZ_00114025">
        <obo:RO_0001025 rdf:resource="http://purl.obolibrary.org/obo/GAZ_00114015"/>
        <obo:IAO_0000115>A commune of Arlit Department.</obo:IAO_0000115>
        <oboInOwl:hasOBONamespace>GAZ</oboInOwl:hasOBONamespace>
        <oboInOwl:id>GAZ:00114025</oboInOwl:id>
        <rdfs:label>Commune of Tchintoulous</rdfs:label>
    </owl:NamedIndividual>
    


    <!-- http://purl.obolibrary.org/obo/GAZ_00114026 -->

    <owl:NamedIndividual rdf:about="http://purl.obolibrary.org/obo/GAZ_00114026">
        <obo:RO_0001025 rdf:resource="http://purl.obolibrary.org/obo/GAZ_00114015"/>
        <obo:IAO_0000115>A commune of Arlit Department.</obo:IAO_0000115>
        <oboInOwl:hasOBONamespace>GAZ</oboInOwl:hasOBONamespace>
        <oboInOwl:id>GAZ:00114026</oboInOwl:id>
        <rdfs:label>Commune of Afassa</rdfs:label>
    </owl:NamedIndividual>
    


    <!-- http://purl.obolibrary.org/obo/GAZ_00114027 -->

    <owl:NamedIndividual rdf:about="http://purl.obolibrary.org/obo/GAZ_00114027">
        <obo:RO_0001025 rdf:resource="http://purl.obolibrary.org/obo/GAZ_00114015"/>
        <obo:IAO_0000115>A commune of Arlit Department.</obo:IAO_0000115>
        <oboInOwl:hasOBONamespace>GAZ</oboInOwl:hasOBONamespace>
        <oboInOwl:id>GAZ:00114027</oboInOwl:id>
        <rdfs:label>Commune of Assarara</rdfs:label>
    </owl:NamedIndividual>
    


    <!-- http://purl.obolibrary.org/obo/GAZ_00114028 -->

    <owl:NamedIndividual rdf:about="http://purl.obolibrary.org/obo/GAZ_00114028">
        <obo:RO_0001025 rdf:resource="http://purl.obolibrary.org/obo/GAZ_00114015"/>
        <obo:IAO_0000115>A commune of Arlit Department.</obo:IAO_0000115>
        <oboInOwl:hasOBONamespace>GAZ</oboInOwl:hasOBONamespace>
        <oboInOwl:id>GAZ:00114028</oboInOwl:id>
        <rdfs:label>Commune of Iferouane</rdfs:label>
    </owl:NamedIndividual>
    


    <!-- http://purl.obolibrary.org/obo/GAZ_00114029 -->

    <owl:NamedIndividual rdf:about="http://purl.obolibrary.org/obo/GAZ_00114029">
        <obo:RO_0001025 rdf:resource="http://purl.obolibrary.org/obo/GAZ_00114015"/>
        <obo:IAO_0000115>A commune of Arlit Department.</obo:IAO_0000115>
        <oboInOwl:hasOBONamespace>GAZ</oboInOwl:hasOBONamespace>
        <oboInOwl:id>GAZ:00114029</oboInOwl:id>
        <rdfs:label>Commune of Sidaouet</rdfs:label>
    </owl:NamedIndividual>
    


    <!-- http://purl.obolibrary.org/obo/GAZ_00114030 -->

    <owl:NamedIndividual rdf:about="http://purl.obolibrary.org/obo/GAZ_00114030">
        <obo:RO_0001025 rdf:resource="http://purl.obolibrary.org/obo/GAZ_00114015"/>
        <obo:IAO_0000115>A commune of Arlit Department.</obo:IAO_0000115>
        <oboInOwl:hasOBONamespace>GAZ</oboInOwl:hasOBONamespace>
        <oboInOwl:id>GAZ:00114030</oboInOwl:id>
        <rdfs:label>Commune of I-n-Azaoua</rdfs:label>
    </owl:NamedIndividual>
    


    <!-- http://purl.obolibrary.org/obo/GAZ_00114031 -->

    <owl:NamedIndividual rdf:about="http://purl.obolibrary.org/obo/GAZ_00114031">
        <obo:RO_0001025 rdf:resource="http://purl.obolibrary.org/obo/GAZ_00114015"/>
        <obo:IAO_0000115>A commune of Arlit Department.</obo:IAO_0000115>
        <oboInOwl:hasOBONamespace>GAZ</oboInOwl:hasOBONamespace>
        <oboInOwl:id>GAZ:00114031</oboInOwl:id>
        <rdfs:label>Commune of Timia</rdfs:label>
    </owl:NamedIndividual>
    


    <!-- http://purl.obolibrary.org/obo/GAZ_00114032 -->

    <owl:NamedIndividual rdf:about="http://purl.obolibrary.org/obo/GAZ_00114032">
        <obo:RO_0001025 rdf:resource="http://purl.obolibrary.org/obo/GAZ_00114015"/>
        <obo:IAO_0000115>A commune of Arlit Department.</obo:IAO_0000115>
        <oboInOwl:hasOBONamespace>GAZ</oboInOwl:hasOBONamespace>
        <oboInOwl:id>GAZ:00114032</oboInOwl:id>
        <rdfs:label>Commune of Aguelal</rdfs:label>
    </owl:NamedIndividual>
    


    <!-- http://purl.obolibrary.org/obo/GAZ_00114033 -->

    <owl:NamedIndividual rdf:about="http://purl.obolibrary.org/obo/GAZ_00114033">
        <obo:RO_0001025 rdf:resource="http://purl.obolibrary.org/obo/GAZ_00032124"/>
        <obo:IAO_0000115>A commune.</obo:IAO_0000115>
        <oboInOwl:hasOBONamespace>GAZ</oboInOwl:hasOBONamespace>
        <oboInOwl:id>GAZ:00114033</oboInOwl:id>
        <rdfs:label>Commune of Guicheme</rdfs:label>
    </owl:NamedIndividual>
    


    <!-- http://purl.obolibrary.org/obo/GAZ_00114034 -->

    <owl:NamedIndividual rdf:about="http://purl.obolibrary.org/obo/GAZ_00114034">
        <obo:RO_0001025 rdf:resource="http://purl.obolibrary.org/obo/GAZ_00032116"/>
        <obo:IAO_0000115>A Communaute Urbaine.</obo:IAO_0000115>
        <oboInOwl:hasOBONamespace>GAZ</oboInOwl:hasOBONamespace>
        <oboInOwl:id>GAZ:00114034</oboInOwl:id>
        <rdfs:label>Communaute Urbaine de Agadaz</rdfs:label>
    </owl:NamedIndividual>
    


    <!-- http://purl.obolibrary.org/obo/GAZ_00114035 -->

    <owl:NamedIndividual rdf:about="http://purl.obolibrary.org/obo/GAZ_00114035">
        <obo:RO_0001025 rdf:resource="http://purl.obolibrary.org/obo/GAZ_00032115"/>
        <obo:IAO_0000115>A commune.</obo:IAO_0000115>
        <oboInOwl:hasOBONamespace>GAZ</oboInOwl:hasOBONamespace>
        <oboInOwl:id>GAZ:00114035</oboInOwl:id>
        <rdfs:label>Commune of Djado</rdfs:label>
    </owl:NamedIndividual>
    


    <!-- http://purl.obolibrary.org/obo/GAZ_00114036 -->

    <owl:NamedIndividual rdf:about="http://purl.obolibrary.org/obo/GAZ_00114036">
        <obo:RO_0001025 rdf:resource="http://purl.obolibrary.org/obo/GAZ_00032115"/>
        <obo:IAO_0000115>A commune.</obo:IAO_0000115>
        <oboInOwl:hasOBONamespace>GAZ</oboInOwl:hasOBONamespace>
        <oboInOwl:id>GAZ:00114036</oboInOwl:id>
        <rdfs:label>Commune of Kawar</rdfs:label>
    </owl:NamedIndividual>
    


    <!-- http://purl.obolibrary.org/obo/GAZ_00114037 -->

    <owl:NamedIndividual rdf:about="http://purl.obolibrary.org/obo/GAZ_00114037">
        <obo:RO_0001025 rdf:resource="http://purl.obolibrary.org/obo/GAZ_00032115"/>
        <obo:IAO_0000115>A Communaute Urbaine.</obo:IAO_0000115>
        <oboInOwl:hasOBONamespace>GAZ</oboInOwl:hasOBONamespace>
        <oboInOwl:id>GAZ:00114037</oboInOwl:id>
        <rdfs:label>Communaute Urbaine de Bilma</rdfs:label>
    </owl:NamedIndividual>
    


    <!-- http://purl.obolibrary.org/obo/GAZ_00114038 -->

    <owl:NamedIndividual rdf:about="http://purl.obolibrary.org/obo/GAZ_00114038">
        <obo:RO_0001025 rdf:resource="http://purl.obolibrary.org/obo/GAZ_00032115"/>
        <obo:IAO_0000115>A commune.</obo:IAO_0000115>
        <oboInOwl:hasOBONamespace>GAZ</oboInOwl:hasOBONamespace>
        <oboInOwl:id>GAZ:00114038</oboInOwl:id>
        <rdfs:label>Commune of Fachi</rdfs:label>
    </owl:NamedIndividual>
    


    <!-- http://purl.obolibrary.org/obo/GAZ_00114039 -->

    <owl:NamedIndividual rdf:about="http://purl.obolibrary.org/obo/GAZ_00114039">
        <obo:RO_0001025 rdf:resource="http://purl.obolibrary.org/obo/GAZ_00032116"/>
        <obo:IAO_0000115>A Communaute Urbaine.</obo:IAO_0000115>
        <oboInOwl:hasOBONamespace>GAZ</oboInOwl:hasOBONamespace>
        <oboInOwl:id>GAZ:00114039</oboInOwl:id>
        <rdfs:label>Communaute Urbaine de Tchirozerine</rdfs:label>
    </owl:NamedIndividual>
    


    <!-- http://purl.obolibrary.org/obo/GAZ_00114040 -->

    <owl:NamedIndividual rdf:about="http://purl.obolibrary.org/obo/GAZ_00114040">
        <obo:RO_0001025 rdf:resource="http://purl.obolibrary.org/obo/GAZ_00032119"/>
        <oboInOwl:hasOBONamespace>GAZ</oboInOwl:hasOBONamespace>
        <oboInOwl:id>GAZ:00114040</oboInOwl:id>
        <rdfs:label>Communaute Urbaine de Nguigmi</rdfs:label>
    </owl:NamedIndividual>
    


    <!-- http://purl.obolibrary.org/obo/GAZ_00114041 -->

    <owl:NamedIndividual rdf:about="http://purl.obolibrary.org/obo/GAZ_00114041">
        <obo:RO_0001025 rdf:resource="http://purl.obolibrary.org/obo/GAZ_00114040"/>
        <obo:IAO_0000115>A national park located in the city of Nguigmi, Niger. Established 1987.</obo:IAO_0000115>
        <oboInOwl:hasOBONamespace>GAZ</oboInOwl:hasOBONamespace>
        <oboInOwl:id>GAZ:00114041</oboInOwl:id>
        <rdfs:label>Abaaba National Park</rdfs:label>
    </owl:NamedIndividual>
    


    <!-- http://purl.obolibrary.org/obo/GAZ_00114042 -->

    <owl:NamedIndividual rdf:about="http://purl.obolibrary.org/obo/GAZ_00114042">
        <obo:RO_0001025 rdf:resource="http://purl.obolibrary.org/obo/GAZ_00000829"/>
        <obo:IAO_0000115>A commune of the city of Niamey.</obo:IAO_0000115>
        <oboInOwl:hasOBONamespace>GAZ</oboInOwl:hasOBONamespace>
        <oboInOwl:id>GAZ:00114042</oboInOwl:id>
        <rdfs:label>Communaute Urbaine de Niamey III</rdfs:label>
    </owl:NamedIndividual>
    


    <!-- http://purl.obolibrary.org/obo/GAZ_00114043 -->

    <owl:NamedIndividual rdf:about="http://purl.obolibrary.org/obo/GAZ_00114043">
        <obo:RO_0001025 rdf:resource="http://purl.obolibrary.org/obo/GAZ_00000829"/>
        <obo:IAO_0000115>A commune of the city of Niamey.</obo:IAO_0000115>
        <oboInOwl:hasOBONamespace>GAZ</oboInOwl:hasOBONamespace>
        <oboInOwl:id>GAZ:00114043</oboInOwl:id>
        <rdfs:label>Communaute Urbaine de Niamey V</rdfs:label>
    </owl:NamedIndividual>
    


    <!-- http://purl.obolibrary.org/obo/GAZ_00114044 -->

    <owl:NamedIndividual rdf:about="http://purl.obolibrary.org/obo/GAZ_00114044">
        <obo:RO_0001025 rdf:resource="http://purl.obolibrary.org/obo/GAZ_00000829"/>
        <obo:IAO_0000115>A commune of the city of Niamey.</obo:IAO_0000115>
        <oboInOwl:hasOBONamespace>GAZ</oboInOwl:hasOBONamespace>
        <oboInOwl:id>GAZ:00114044</oboInOwl:id>
        <rdfs:label>Communaute Urbaine de Niamey I</rdfs:label>
    </owl:NamedIndividual>
    


    <!-- http://purl.obolibrary.org/obo/GAZ_00114045 -->

    <owl:NamedIndividual rdf:about="http://purl.obolibrary.org/obo/GAZ_00114045">
        <obo:RO_0001025 rdf:resource="http://purl.obolibrary.org/obo/GAZ_00000829"/>
        <obo:IAO_0000115>A commune of the city of Niamey.</obo:IAO_0000115>
        <oboInOwl:hasOBONamespace>GAZ</oboInOwl:hasOBONamespace>
        <oboInOwl:id>GAZ:00114045</oboInOwl:id>
        <rdfs:label>Communaute Urbaine de Niamey II</rdfs:label>
    </owl:NamedIndividual>
    


    <!-- http://purl.obolibrary.org/obo/GAZ_00114046 -->

    <owl:NamedIndividual rdf:about="http://purl.obolibrary.org/obo/GAZ_00114046">
        <obo:RO_0001025 rdf:resource="http://purl.obolibrary.org/obo/GAZ_00000829"/>
        <obo:IAO_0000115>A commune of the city of Niamey.</obo:IAO_0000115>
        <oboInOwl:hasOBONamespace>GAZ</oboInOwl:hasOBONamespace>
        <oboInOwl:id>GAZ:00114046</oboInOwl:id>
        <rdfs:label>Communaute Urbaine de Niamey IV</rdfs:label>
    </owl:NamedIndividual>
    


    <!-- http://purl.obolibrary.org/obo/GAZ_00122801 -->

    <owl:NamedIndividual rdf:about="http://purl.obolibrary.org/obo/GAZ_00122801">
        <obo:IAO_0000115>A depression located at the southern edge of the Sahara Desert in north central Africa, is the lowest point in Chad, and one of the largest sources of airborne dust in the world. Once serving as part of the floor of a much larger Lake Chad.</obo:IAO_0000115>
        <oboInOwl:hasOBONamespace>GAZ</oboInOwl:hasOBONamespace>
        <oboInOwl:id>GAZ:00122801</oboInOwl:id>
        <rdfs:label>Bodele Depression</rdfs:label>
    </owl:NamedIndividual>
    


    <!-- http://purl.obolibrary.org/obo/GAZ_00147864 -->

    <owl:NamedIndividual rdf:about="http://purl.obolibrary.org/obo/GAZ_00147864">
        <obo:IAO_0000115>A large area of lakes and floodplains in Mali. It is located in the middle course of the Niger River, between the bifurcated Niger and its tributary, the Bani. Cities such as Mopti, Sevare and Djenne lie in the 400 km-long region.</obo:IAO_0000115>
        <oboInOwl:hasOBONamespace>GAZ</oboInOwl:hasOBONamespace>
        <oboInOwl:id>GAZ:00147864</oboInOwl:id>
        <rdfs:label>Niger Inland Delta</rdfs:label>
    </owl:NamedIndividual>
    


    <!-- http://purl.obolibrary.org/obo/GAZ_00230221 -->

    <owl:NamedIndividual rdf:about="http://purl.obolibrary.org/obo/GAZ_00230221">
        <obo:IAO_0000115>A lake in Chad and Cameroon. It does not have clearly delineated borders, as it forms the western border of an area of permanent swampland. The lake forms with the seasonal flooding of the Logone River. A channel connects the northern end of the lake with the Logone River and another connects the southern end with the River Kebbi.</obo:IAO_0000115>
        <oboInOwl:hasOBONamespace>GAZ</oboInOwl:hasOBONamespace>
        <oboInOwl:id>GAZ:00230221</oboInOwl:id>
        <rdfs:label>Lake Fianga</rdfs:label>
    </owl:NamedIndividual>
    


    <!-- http://purl.obolibrary.org/obo/GAZ_00230227 -->

    <owl:NamedIndividual rdf:about="http://purl.obolibrary.org/obo/GAZ_00230227">
        <obo:IAO_0000115>A man-made lake located in the Northern Region of Cameroon. It is located 50 km south of the city of Garoua on the Benue River. Constructed 1977-1982.</obo:IAO_0000115>
        <oboInOwl:hasOBONamespace>GAZ</oboInOwl:hasOBONamespace>
        <oboInOwl:id>GAZ:00230227</oboInOwl:id>
        <rdfs:label>Lagdo Reservoir</rdfs:label>
    </owl:NamedIndividual>
    


    <!-- http://purl.obolibrary.org/obo/GAZ_00230241 -->

    <owl:NamedIndividual rdf:about="http://purl.obolibrary.org/obo/GAZ_00230241">
        <obo:IAO_0000115>A river. A tributary of the Logone River.</obo:IAO_0000115>
        <oboInOwl:hasOBONamespace>GAZ</oboInOwl:hasOBONamespace>
        <oboInOwl:id>GAZ:00230241</oboInOwl:id>
        <rdfs:label>Tandjile River</rdfs:label>
    </owl:NamedIndividual>
    


    <!-- http://purl.obolibrary.org/obo/GAZ_00230256 -->

    <owl:NamedIndividual rdf:about="http://purl.obolibrary.org/obo/GAZ_00230256">
        <obo:IAO_0000115>Two lakes on the Chad/Cameroon border.</obo:IAO_0000115>
        <oboInOwl:hasOBONamespace>GAZ</oboInOwl:hasOBONamespace>
        <oboInOwl:id>GAZ:00230256</oboInOwl:id>
        <rdfs:label>Lacs Lere</rdfs:label>
    </owl:NamedIndividual>
    


    <!-- http://purl.obolibrary.org/obo/GAZ_00230302 -->

    <owl:NamedIndividual rdf:about="http://purl.obolibrary.org/obo/GAZ_00230302">
        <obo:RO_0001025 rdf:resource="http://purl.obolibrary.org/obo/GAZ_00009949"/>
        <obo:IAO_0000115>An irrigation canal. Cosntructed 1873.</obo:IAO_0000115>
        <oboInOwl:hasOBONamespace>GAZ</oboInOwl:hasOBONamespace>
        <oboInOwl:id>GAZ:00230302</oboInOwl:id>
        <rdfs:label>Ibrahimiya Canal</rdfs:label>
    </owl:NamedIndividual>
    


    <!-- http://purl.obolibrary.org/obo/GAZ_00230306 -->

    <owl:NamedIndividual rdf:about="http://purl.obolibrary.org/obo/GAZ_00230306">
        <obo:RO_0001025 rdf:resource="http://purl.obolibrary.org/obo/GAZ_00230307"/>
        <obo:IAO_0000115>A mountain range in the area of the Egyptian-Libyan-Sudanese border.</obo:IAO_0000115>
        <oboInOwl:hasOBONamespace>GAZ</oboInOwl:hasOBONamespace>
        <oboInOwl:id>GAZ:00230306</oboInOwl:id>
        <rdfs:label>Jebel Uweinat</rdfs:label>
    </owl:NamedIndividual>
    


    <!-- http://purl.obolibrary.org/obo/GAZ_00230307 -->

    <owl:NamedIndividual rdf:about="http://purl.obolibrary.org/obo/GAZ_00230307">
        <obo:IAO_0000115>A plateau in the remote southwest corner of Egypt.</obo:IAO_0000115>
        <oboInOwl:hasOBONamespace>GAZ</oboInOwl:hasOBONamespace>
        <oboInOwl:id>GAZ:00230307</oboInOwl:id>
        <rdfs:label>Gilf Kebir</rdfs:label>
    </owl:NamedIndividual>
    


    <!-- http://purl.obolibrary.org/obo/GAZ_00230308 -->

    <owl:NamedIndividual rdf:about="http://purl.obolibrary.org/obo/GAZ_00230308">
        <obo:RO_0001025 rdf:resource="http://purl.obolibrary.org/obo/GAZ_00230307"/>
        <obo:IAO_0000115>An impact crater.</obo:IAO_0000115>
        <oboInOwl:hasOBONamespace>GAZ</oboInOwl:hasOBONamespace>
        <oboInOwl:id>GAZ:00230308</oboInOwl:id>
        <rdfs:label>Kebira Crater</rdfs:label>
    </owl:NamedIndividual>
    


    <!-- http://purl.obolibrary.org/obo/GAZ_00230309 -->

    <owl:NamedIndividual rdf:about="http://purl.obolibrary.org/obo/GAZ_00230309">
        <obo:RO_0001025 rdf:resource="http://purl.obolibrary.org/obo/GAZ_00230307"/>
        <obo:IAO_0000115>A dry river bed.</obo:IAO_0000115>
        <oboInOwl:hasOBONamespace>GAZ</oboInOwl:hasOBONamespace>
        <oboInOwl:id>GAZ:00230309</oboInOwl:id>
        <rdfs:label>Wadi Akhdar</rdfs:label>
    </owl:NamedIndividual>
    


    <!-- http://purl.obolibrary.org/obo/GAZ_00230310 -->

    <owl:NamedIndividual rdf:about="http://purl.obolibrary.org/obo/GAZ_00230310">
        <obo:RO_0001025 rdf:resource="http://purl.obolibrary.org/obo/GAZ_00230307"/>
        <obo:IAO_0000115>A dry river bed.</obo:IAO_0000115>
        <oboInOwl:hasOBONamespace>GAZ</oboInOwl:hasOBONamespace>
        <oboInOwl:id>GAZ:00230310</oboInOwl:id>
        <rdfs:label>Wadi Bakht</rdfs:label>
    </owl:NamedIndividual>
    


    <!-- http://purl.obolibrary.org/obo/GAZ_00230311 -->

    <owl:NamedIndividual rdf:about="http://purl.obolibrary.org/obo/GAZ_00230311">
        <obo:RO_0001025 rdf:resource="http://purl.obolibrary.org/obo/GAZ_00230307"/>
        <obo:IAO_0000115>A dry river bed.</obo:IAO_0000115>
        <oboInOwl:hasOBONamespace>GAZ</oboInOwl:hasOBONamespace>
        <oboInOwl:id>GAZ:00230311</oboInOwl:id>
        <rdfs:label>Wadi Dayiq</rdfs:label>
    </owl:NamedIndividual>
    


    <!-- http://purl.obolibrary.org/obo/GAZ_00230312 -->

    <owl:NamedIndividual rdf:about="http://purl.obolibrary.org/obo/GAZ_00230312">
        <obo:RO_0001025 rdf:resource="http://purl.obolibrary.org/obo/GAZ_00230307"/>
        <obo:IAO_0000115>A dry river bed.</obo:IAO_0000115>
        <oboInOwl:hasOBONamespace>GAZ</oboInOwl:hasOBONamespace>
        <oboInOwl:id>GAZ:00230312</oboInOwl:id>
        <rdfs:label>Wadi Firaq</rdfs:label>
    </owl:NamedIndividual>
    


    <!-- http://purl.obolibrary.org/obo/GAZ_00230313 -->

    <owl:NamedIndividual rdf:about="http://purl.obolibrary.org/obo/GAZ_00230313">
        <obo:RO_0001025 rdf:resource="http://purl.obolibrary.org/obo/GAZ_00230307"/>
        <obo:IAO_0000115>A dry river bed.</obo:IAO_0000115>
        <oboInOwl:hasOBONamespace>GAZ</oboInOwl:hasOBONamespace>
        <oboInOwl:id>GAZ:00230313</oboInOwl:id>
        <rdfs:label>Wadi Gazayir</rdfs:label>
    </owl:NamedIndividual>
    


    <!-- http://purl.obolibrary.org/obo/GAZ_00230314 -->

    <owl:NamedIndividual rdf:about="http://purl.obolibrary.org/obo/GAZ_00230314">
        <obo:RO_0001025 rdf:resource="http://purl.obolibrary.org/obo/GAZ_00230307"/>
        <obo:IAO_0000115>A dry river bed.</obo:IAO_0000115>
        <oboInOwl:hasOBONamespace>GAZ</oboInOwl:hasOBONamespace>
        <oboInOwl:id>GAZ:00230314</oboInOwl:id>
        <rdfs:label>Wadi Maftuh</rdfs:label>
    </owl:NamedIndividual>
    


    <!-- http://purl.obolibrary.org/obo/GAZ_00230315 -->

    <owl:NamedIndividual rdf:about="http://purl.obolibrary.org/obo/GAZ_00230315">
        <obo:RO_0001025 rdf:resource="http://purl.obolibrary.org/obo/GAZ_00230307"/>
        <obo:IAO_0000115>A dry river bed.</obo:IAO_0000115>
        <oboInOwl:hasOBONamespace>GAZ</oboInOwl:hasOBONamespace>
        <oboInOwl:id>GAZ:00230315</oboInOwl:id>
        <rdfs:label>Wadi Mashi</rdfs:label>
    </owl:NamedIndividual>
    


    <!-- http://purl.obolibrary.org/obo/GAZ_00230316 -->

    <owl:NamedIndividual rdf:about="http://purl.obolibrary.org/obo/GAZ_00230316">
        <obo:RO_0001025 rdf:resource="http://purl.obolibrary.org/obo/GAZ_00230307"/>
        <obo:IAO_0000115>A dry river bed.</obo:IAO_0000115>
        <oboInOwl:hasOBONamespace>GAZ</oboInOwl:hasOBONamespace>
        <oboInOwl:id>GAZ:00230316</oboInOwl:id>
        <rdfs:label>Wadi Sura</rdfs:label>
    </owl:NamedIndividual>
    


    <!-- http://purl.obolibrary.org/obo/GAZ_00230317 -->

    <owl:NamedIndividual rdf:about="http://purl.obolibrary.org/obo/GAZ_00230317">
        <obo:RO_0001025 rdf:resource="http://purl.obolibrary.org/obo/GAZ_00230307"/>
        <obo:IAO_0000115>A dry river bed.</obo:IAO_0000115>
        <oboInOwl:hasOBONamespace>GAZ</oboInOwl:hasOBONamespace>
        <oboInOwl:id>GAZ:00230317</oboInOwl:id>
        <rdfs:label>Wadi Wassa</rdfs:label>
    </owl:NamedIndividual>
    


    <!-- http://purl.obolibrary.org/obo/GAZ_00230323 -->

    <owl:NamedIndividual rdf:about="http://purl.obolibrary.org/obo/GAZ_00230323">
        <obo:RO_0001025 rdf:resource="http://purl.obolibrary.org/obo/GAZ_00230307"/>
        <obo:IAO_0000115>A cave in southwest Egypt, near the border with Libya, in the mountainous Gilf Kebir region of the Sahara Desert.</obo:IAO_0000115>
        <oboInOwl:hasOBONamespace>GAZ</oboInOwl:hasOBONamespace>
        <oboInOwl:id>GAZ:00230323</oboInOwl:id>
        <rdfs:label>Cave of Swimmers</rdfs:label>
    </owl:NamedIndividual>
    


    <!-- http://purl.obolibrary.org/obo/GAZ_00230324 -->

    <owl:NamedIndividual rdf:about="http://purl.obolibrary.org/obo/GAZ_00230324">
        <obo:RO_0001025 rdf:resource="http://purl.obolibrary.org/obo/GAZ_00058890"/>
        <obo:IAO_0000115>An island in the first cataract of the Nile River, Egypt.</obo:IAO_0000115>
        <oboInOwl:hasOBONamespace>GAZ</oboInOwl:hasOBONamespace>
        <oboInOwl:id>GAZ:00230324</oboInOwl:id>
        <rdfs:label>Bigeh</rdfs:label>
    </owl:NamedIndividual>
    


    <!-- http://purl.obolibrary.org/obo/GAZ_00230325 -->

    <owl:NamedIndividual rdf:about="http://purl.obolibrary.org/obo/GAZ_00230325">
        <obo:IAO_0000115>An island in the River Nile, located just downstream of the First Cataract.</obo:IAO_0000115>
        <oboInOwl:hasOBONamespace>GAZ</oboInOwl:hasOBONamespace>
        <oboInOwl:id>GAZ:00230325</oboInOwl:id>
        <rdfs:label>Elephantine</rdfs:label>
    </owl:NamedIndividual>
    


    <!-- http://purl.obolibrary.org/obo/GAZ_00230326 -->

    <owl:NamedIndividual rdf:about="http://purl.obolibrary.org/obo/GAZ_00230326">
        <obo:IAO_0000115>An island located in the Nile River, in central Cairo.</obo:IAO_0000115>
        <oboInOwl:hasOBONamespace>GAZ</oboInOwl:hasOBONamespace>
        <oboInOwl:id>GAZ:00230326</oboInOwl:id>
        <rdfs:label>Gezira Island</rdfs:label>
    </owl:NamedIndividual>
    


    <!-- http://purl.obolibrary.org/obo/GAZ_00230327 -->

    <owl:NamedIndividual rdf:about="http://purl.obolibrary.org/obo/GAZ_00230327">
        <obo:IAO_0000115>An oval-shaped island in the Nile at Aswan, Egypt.</obo:IAO_0000115>
        <oboInOwl:hasOBONamespace>GAZ</oboInOwl:hasOBONamespace>
        <oboInOwl:id>GAZ:00230327</oboInOwl:id>
        <rdfs:label>Geziret an-Nabatat</rdfs:label>
    </owl:NamedIndividual>
    


    <!-- http://purl.obolibrary.org/obo/GAZ_00230398 -->

    <owl:NamedIndividual rdf:about="http://purl.obolibrary.org/obo/GAZ_00230398">
        <obo:IAO_0000115>A river. A tributary of the Jamma River. Along with the Adabay River, it defined the border of the former district of Marra Biete.</obo:IAO_0000115>
        <oboInOwl:hasOBONamespace>GAZ</oboInOwl:hasOBONamespace>
        <oboInOwl:id>GAZ:00230398</oboInOwl:id>
        <rdfs:label>Wanchet River</rdfs:label>
    </owl:NamedIndividual>
    


    <!-- http://purl.obolibrary.org/obo/GAZ_00230400 -->

    <owl:NamedIndividual rdf:about="http://purl.obolibrary.org/obo/GAZ_00230400">
        <obo:IAO_0000115>A river in Sudan, Africa. The most southerly of the great eastern tributaries of the Nile, the Sobat enters the White Nile at Dolieb Hill, near the city of Malakal in the Upper Nile state of Sudan.</obo:IAO_0000115>
        <oboInOwl:hasOBONamespace>GAZ</oboInOwl:hasOBONamespace>
        <oboInOwl:id>GAZ:00230400</oboInOwl:id>
        <rdfs:label>Sobat River</rdfs:label>
    </owl:NamedIndividual>
    


    <!-- http://purl.obolibrary.org/obo/GAZ_00230410 -->

    <owl:NamedIndividual rdf:about="http://purl.obolibrary.org/obo/GAZ_00230410">
        <obo:IAO_0000115>A river of southwestern Ethiopia. It is a tributary of the Baro River.</obo:IAO_0000115>
        <oboInOwl:hasOBONamespace>GAZ</oboInOwl:hasOBONamespace>
        <oboInOwl:id>GAZ:00230410</oboInOwl:id>
        <rdfs:label>Jikawo River</rdfs:label>
    </owl:NamedIndividual>
    


    <!-- http://purl.obolibrary.org/obo/GAZ_00230416 -->

    <owl:NamedIndividual rdf:about="http://purl.obolibrary.org/obo/GAZ_00230416">
        <obo:IAO_0000115>A dam. Constructed 1986.</obo:IAO_0000115>
        <oboInOwl:hasOBONamespace>GAZ</oboInOwl:hasOBONamespace>
        <oboInOwl:id>GAZ:00230416</oboInOwl:id>
        <rdfs:label>Angereb Dam</rdfs:label>
    </owl:NamedIndividual>
    


    <!-- http://purl.obolibrary.org/obo/GAZ_00230530 -->

    <owl:NamedIndividual rdf:about="http://purl.obolibrary.org/obo/GAZ_00230530">
        <obo:IAO_0000115>A valley in west-central Libya, arising out of the Sawda Mountains, situated between the towns Wanzarik and Umm al-&apos;Abid in the west and east, respectively.</obo:IAO_0000115>
        <oboInOwl:hasOBONamespace>GAZ</oboInOwl:hasOBONamespace>
        <oboInOwl:id>GAZ:00230530</oboInOwl:id>
        <rdfs:label>Wadi ash-Shati&apos;</rdfs:label>
    </owl:NamedIndividual>
    


    <!-- http://purl.obolibrary.org/obo/GAZ_00230531 -->

    <owl:NamedIndividual rdf:about="http://purl.obolibrary.org/obo/GAZ_00230531">
        <obo:IAO_0000115>A primarily erg desert in southwestern Libya and is considered part of the Sahara desert complex, although it is separated from the southern Sahara by the Tibesti Mountains and the Tassili n&apos;Ajjer.</obo:IAO_0000115>
        <oboInOwl:hasOBONamespace>GAZ</oboInOwl:hasOBONamespace>
        <oboInOwl:id>GAZ:00230531</oboInOwl:id>
        <rdfs:label>Murzuq Desert</rdfs:label>
    </owl:NamedIndividual>
    


    <!-- http://purl.obolibrary.org/obo/GAZ_00230545 -->

    <owl:NamedIndividual rdf:about="http://purl.obolibrary.org/obo/GAZ_00230545">
        <obo:IAO_0000115>An erg located in the far south-east of Western Sahara.</obo:IAO_0000115>
        <oboInOwl:hasOBONamespace>GAZ</oboInOwl:hasOBONamespace>
        <oboInOwl:id>GAZ:00230545</oboInOwl:id>
        <rdfs:label>Zug</rdfs:label>
    </owl:NamedIndividual>
    


    <!-- http://purl.obolibrary.org/obo/GAZ_00230712 -->

    <owl:NamedIndividual rdf:about="http://purl.obolibrary.org/obo/GAZ_00230712">
        <obo:IAO_0000115>A sandstone massif in Mali&apos;s Kidal Region.</obo:IAO_0000115>
        <oboInOwl:hasOBONamespace>GAZ</oboInOwl:hasOBONamespace>
        <oboInOwl:id>GAZ:00230712</oboInOwl:id>
        <rdfs:label>Adrar des Ifoghas</rdfs:label>
    </owl:NamedIndividual>
    


    <!-- http://purl.obolibrary.org/obo/GAZ_00230726 -->

    <owl:NamedIndividual rdf:about="http://purl.obolibrary.org/obo/GAZ_00230726">
        <obo:IAO_0000115>A hydroelectric dam located in the Koulikoro Region, on the Sankarani River. Impounds Lake Selingue. Constructed 1979-1982.</obo:IAO_0000115>
        <oboInOwl:hasOBONamespace>GAZ</oboInOwl:hasOBONamespace>
        <oboInOwl:id>GAZ:00230726</oboInOwl:id>
        <rdfs:label>Selingue Dam</rdfs:label>
    </owl:NamedIndividual>
    


    <!-- http://purl.obolibrary.org/obo/GAZ_00230727 -->

    <owl:NamedIndividual rdf:about="http://purl.obolibrary.org/obo/GAZ_00230727">
        <obo:IAO_0000115>A man-made lake impounded by Selingue Dam. Constructed 1979-1982.</obo:IAO_0000115>
        <oboInOwl:hasOBONamespace>GAZ</oboInOwl:hasOBONamespace>
        <oboInOwl:id>GAZ:00230727</oboInOwl:id>
        <rdfs:label>Lake Selingue</rdfs:label>
    </owl:NamedIndividual>
    


    <!-- http://purl.obolibrary.org/obo/GAZ_00230845 -->

    <owl:NamedIndividual rdf:about="http://purl.obolibrary.org/obo/GAZ_00230845">
        <obo:RO_0001025 rdf:resource="http://purl.obolibrary.org/obo/GAZ_00147864"/>
        <obo:IAO_0000115>A Ramsar site.</obo:IAO_0000115>
        <oboInOwl:hasOBONamespace>GAZ</oboInOwl:hasOBONamespace>
        <oboInOwl:id>GAZ:00230845</oboInOwl:id>
        <rdfs:label>Walado Debo</rdfs:label>
    </owl:NamedIndividual>
    


    <!-- http://purl.obolibrary.org/obo/GAZ_00230846 -->

    <owl:NamedIndividual rdf:about="http://purl.obolibrary.org/obo/GAZ_00230846">
        <obo:RO_0001025 rdf:resource="http://purl.obolibrary.org/obo/GAZ_00147864"/>
        <obo:IAO_0000115>A lake. A Ramsar Site.</obo:IAO_0000115>
        <oboInOwl:hasOBONamespace>GAZ</oboInOwl:hasOBONamespace>
        <oboInOwl:id>GAZ:00230846</oboInOwl:id>
        <rdfs:label>Lake Horo</rdfs:label>
    </owl:NamedIndividual>
    


    <!-- http://purl.obolibrary.org/obo/GAZ_00230847 -->

    <owl:NamedIndividual rdf:about="http://purl.obolibrary.org/obo/GAZ_00230847">
        <obo:RO_0001025 rdf:resource="http://purl.obolibrary.org/obo/GAZ_00147864"/>
        <obo:IAO_0000115>A Ramsar Site.</obo:IAO_0000115>
        <oboInOwl:hasOBONamespace>GAZ</oboInOwl:hasOBONamespace>
        <oboInOwl:id>GAZ:00230847</oboInOwl:id>
        <rdfs:label>Plaine de Seri</rdfs:label>
    </owl:NamedIndividual>
    


    <!-- http://purl.obolibrary.org/obo/GAZ_00231580 -->

    <owl:NamedIndividual rdf:about="http://purl.obolibrary.org/obo/GAZ_00231580">
        <obo:IAO_0000115>A plateau that lies in eastern Mauritania, forming a stony part of the Sahara Desert.</obo:IAO_0000115>
        <oboInOwl:hasOBONamespace>GAZ</oboInOwl:hasOBONamespace>
        <oboInOwl:id>GAZ:00231580</oboInOwl:id>
        <rdfs:label>Tagant Plateau</rdfs:label>
    </owl:NamedIndividual>
    


    <!-- http://purl.obolibrary.org/obo/GAZ_00231625 -->

    <owl:NamedIndividual rdf:about="http://purl.obolibrary.org/obo/GAZ_00231625">
        <obo:IAO_0000115>A highland area of the Sahara Desert in northern Mauritania.</obo:IAO_0000115>
        <oboInOwl:hasOBONamespace>GAZ</oboInOwl:hasOBONamespace>
        <oboInOwl:id>GAZ:00231625</oboInOwl:id>
        <rdfs:label>Adrar Plateau</rdfs:label>
    </owl:NamedIndividual>
    


    <!-- http://purl.obolibrary.org/obo/GAZ_00233398 -->

    <owl:NamedIndividual rdf:about="http://purl.obolibrary.org/obo/GAZ_00233398">
        <obo:IAO_0000115>The N area of the Termit Massif.</obo:IAO_0000115>
        <oboInOwl:hasOBONamespace>GAZ</oboInOwl:hasOBONamespace>
        <oboInOwl:id>GAZ:00233398</oboInOwl:id>
        <rdfs:label>Gossololom</rdfs:label>
    </owl:NamedIndividual>
    


    <!-- http://purl.obolibrary.org/obo/GAZ_00233399 -->

    <owl:NamedIndividual rdf:about="http://purl.obolibrary.org/obo/GAZ_00233399">
        <obo:IAO_0000115>Foothills of the Termit Massif to the SW.</obo:IAO_0000115>
        <oboInOwl:hasOBONamespace>GAZ</oboInOwl:hasOBONamespace>
        <oboInOwl:id>GAZ:00233399</oboInOwl:id>
        <rdfs:label>Koutous Hills</rdfs:label>
    </owl:NamedIndividual>
    


    <!-- http://purl.obolibrary.org/obo/GAZ_00233400 -->

    <owl:NamedIndividual rdf:about="http://purl.obolibrary.org/obo/GAZ_00233400">
        <obo:IAO_0000115>A protected area. Established 1962-01-01.</obo:IAO_0000115>
        <oboInOwl:hasOBONamespace>GAZ</oboInOwl:hasOBONamespace>
        <oboInOwl:id>GAZ:00233400</oboInOwl:id>
        <rdfs:label>Termit Massif Reserve</rdfs:label>
    </owl:NamedIndividual>
    


    <!-- http://purl.obolibrary.org/obo/GAZ_00233401 -->

    <owl:NamedIndividual rdf:about="http://purl.obolibrary.org/obo/GAZ_00233401">
        <obo:RO_0001025 rdf:resource="http://purl.obolibrary.org/obo/GAZ_00233400"/>
        <obo:IAO_0000115>A protected area. It forms a half ring around the southern border of the larger Termit Massif Total Reserve.</obo:IAO_0000115>
        <oboInOwl:hasOBONamespace>GAZ</oboInOwl:hasOBONamespace>
        <oboInOwl:id>GAZ:00233401</oboInOwl:id>
        <rdfs:label>Termit Massif Faunal Reserve Buffer Zone</rdfs:label>
    </owl:NamedIndividual>
    


    <!-- http://purl.obolibrary.org/obo/GAZ_00233402 -->

    <owl:NamedIndividual rdf:about="http://purl.obolibrary.org/obo/GAZ_00233402">
        <obo:RO_0001025 rdf:resource="http://purl.obolibrary.org/obo/GAZ_00233400"/>
        <obo:IAO_0000115>A protected area.</obo:IAO_0000115>
        <oboInOwl:hasOBONamespace>GAZ</oboInOwl:hasOBONamespace>
        <oboInOwl:id>GAZ:00233402</oboInOwl:id>
        <rdfs:label>Termit Massif Total Reserve</rdfs:label>
    </owl:NamedIndividual>
    


    <!-- http://purl.obolibrary.org/obo/GAZ_00233403 -->

    <owl:NamedIndividual rdf:about="http://purl.obolibrary.org/obo/GAZ_00233403">
        <obo:RO_0001025 rdf:resource="http://purl.obolibrary.org/obo/GAZ_00000827"/>
        <obo:IAO_0000115>A protected area. Established 1962-01-01.</obo:IAO_0000115>
        <oboInOwl:hasOBONamespace>GAZ</oboInOwl:hasOBONamespace>
        <oboInOwl:id>GAZ:00233403</oboInOwl:id>
        <rdfs:label>Tamou Reserve</rdfs:label>
    </owl:NamedIndividual>
    


    <!-- http://purl.obolibrary.org/obo/GAZ_00233404 -->

    <owl:NamedIndividual rdf:about="http://purl.obolibrary.org/obo/GAZ_00233404">
        <obo:RO_0001025 rdf:resource="http://purl.obolibrary.org/obo/GAZ_00000822"/>
        <obo:IAO_0000115>A protected area.</obo:IAO_0000115>
        <oboInOwl:hasOBONamespace>GAZ</oboInOwl:hasOBONamespace>
        <oboInOwl:id>GAZ:00233404</oboInOwl:id>
        <rdfs:label>Tadres Total Reserve</rdfs:label>
    </owl:NamedIndividual>
    


    <!-- http://purl.obolibrary.org/obo/GAZ_00233405 -->

    <owl:NamedIndividual rdf:about="http://purl.obolibrary.org/obo/GAZ_00233405">
        <obo:RO_0001025 rdf:resource="http://purl.obolibrary.org/obo/GAZ_00000825"/>
        <obo:IAO_0000115>A protected area located within the northern tip of the Maradi Region, just north of the town of Dakoro, and south of the border with the Agadez Region. Established 1955-01-01.</obo:IAO_0000115>
        <oboInOwl:hasOBONamespace>GAZ</oboInOwl:hasOBONamespace>
        <oboInOwl:id>GAZ:00233405</oboInOwl:id>
        <rdfs:label>Gadabedji Total Reserve</rdfs:label>
    </owl:NamedIndividual>
    


    <!-- http://purl.obolibrary.org/obo/GAZ_00233406 -->

    <owl:NamedIndividual rdf:about="http://purl.obolibrary.org/obo/GAZ_00233406">
        <obo:RO_0001025 rdf:resource="http://purl.obolibrary.org/obo/GAZ_00000824"/>
        <obo:IAO_0000115>A protected area located n the mouth of Dallol Bosso valley. Established 1962-01-01.</obo:IAO_0000115>
        <oboInOwl:hasOBONamespace>GAZ</oboInOwl:hasOBONamespace>
        <oboInOwl:id>GAZ:00233406</oboInOwl:id>
        <rdfs:label>Dosso Partial Faunal Reserve</rdfs:label>
    </owl:NamedIndividual>
    


    <!-- http://purl.obolibrary.org/obo/GAZ_00233408 -->

    <owl:NamedIndividual rdf:about="http://purl.obolibrary.org/obo/GAZ_00233408">
        <obo:RO_0001025 rdf:resource="http://purl.obolibrary.org/obo/GAZ_00000822"/>
        <obo:IAO_0000115>A protected area. Established 1988-01-01.</obo:IAO_0000115>
        <oboInOwl:hasOBONamespace>GAZ</oboInOwl:hasOBONamespace>
        <oboInOwl:id>GAZ:00233408</oboInOwl:id>
        <rdfs:label>Air and Tenere Addax Sanctuary</rdfs:label>
    </owl:NamedIndividual>
    


    <!-- http://purl.obolibrary.org/obo/GAZ_00233409 -->

    <owl:NamedIndividual rdf:about="http://purl.obolibrary.org/obo/GAZ_00233409">
        <obo:RO_0001025 rdf:resource="http://purl.obolibrary.org/obo/GAZ_00000585"/>
        <obo:IAO_0000115>A protected area. It includes both the eastern half of the Air Mountains and the western sections of the Tenere desert.</obo:IAO_0000115>
        <oboInOwl:hasOBONamespace>GAZ</oboInOwl:hasOBONamespace>
        <oboInOwl:id>GAZ:00233409</oboInOwl:id>
        <rdfs:label>Air and Tenere National Nature Reserve</rdfs:label>
    </owl:NamedIndividual>
    


    <!-- http://purl.obolibrary.org/obo/GAZ_00233410 -->

    <owl:NamedIndividual rdf:about="http://purl.obolibrary.org/obo/GAZ_00233410">
        <obo:RO_0001025 rdf:resource="http://purl.obolibrary.org/obo/GAZ_00000824"/>
        <obo:IAO_0000115>An island in the River Niger about. 16 km long and 4 km wide, located around 40 km from the town of Gaya, Niger.</obo:IAO_0000115>
        <oboInOwl:hasOBONamespace>GAZ</oboInOwl:hasOBONamespace>
        <oboInOwl:id>GAZ:00233410</oboInOwl:id>
        <rdfs:label>Lete Island</rdfs:label>
    </owl:NamedIndividual>
    


    <!-- http://purl.obolibrary.org/obo/GAZ_00233411 -->

    <owl:NamedIndividual rdf:about="http://purl.obolibrary.org/obo/GAZ_00233411">
        <obo:RO_0001025 rdf:resource="http://purl.obolibrary.org/obo/GAZ_00114015"/>
        <obo:IAO_0000115>A plateau that ies in the Sahara, in north eastern Niger.</obo:IAO_0000115>
        <oboInOwl:hasOBONamespace>GAZ</oboInOwl:hasOBONamespace>
        <oboInOwl:id>GAZ:00233411</oboInOwl:id>
        <rdfs:label>Djado Plateau</rdfs:label>
    </owl:NamedIndividual>
    


    <!-- http://purl.obolibrary.org/obo/GAZ_00233412 -->

    <owl:NamedIndividual rdf:about="http://purl.obolibrary.org/obo/GAZ_00233412">
        <obo:RO_0001025 rdf:resource="http://purl.obolibrary.org/obo/GAZ_00103898"/>
        <obo:RO_0001025 rdf:resource="http://purl.obolibrary.org/obo/GAZ_00233408"/>
        <obo:IAO_0000115>A mountain range in Niger in the northeastern section of the Air Massif, about 100 km ENE of the town of Iferouane and 30 km NE of the Tezerik oasis. Isolated from the main Massif by dune seas of the Erg of Tenere and a flat gravely Desert pavement plain.</obo:IAO_0000115>
        <oboInOwl:hasOBONamespace>GAZ</oboInOwl:hasOBONamespace>
        <oboInOwl:id>GAZ:00233412</oboInOwl:id>
        <rdfs:label>Montagnes Bleus</rdfs:label>
    </owl:NamedIndividual>
    


    <!-- http://purl.obolibrary.org/obo/GAZ_00233422 -->

    <owl:NamedIndividual rdf:about="http://purl.obolibrary.org/obo/GAZ_00233422">
        <obo:IAO_0000115>A lake.</obo:IAO_0000115>
        <oboInOwl:hasOBONamespace>GAZ</oboInOwl:hasOBONamespace>
        <oboInOwl:id>GAZ:00233422</oboInOwl:id>
        <rdfs:label>Nguru Lake</rdfs:label>
    </owl:NamedIndividual>
    


    <!-- http://purl.obolibrary.org/obo/GAZ_00233424 -->

    <owl:NamedIndividual rdf:about="http://purl.obolibrary.org/obo/GAZ_00233424">
        <obo:IAO_0000115>A dam. Impounds Challawa Gorge Reservoir. Constructed 1990-1992.</obo:IAO_0000115>
        <oboInOwl:hasOBONamespace>GAZ</oboInOwl:hasOBONamespace>
        <oboInOwl:id>GAZ:00233424</oboInOwl:id>
        <rdfs:label>Challawa Gorge Dam</rdfs:label>
    </owl:NamedIndividual>
    


    <!-- http://purl.obolibrary.org/obo/GAZ_00233425 -->

    <owl:NamedIndividual rdf:about="http://purl.obolibrary.org/obo/GAZ_00233425">
        <obo:IAO_0000115>A reservoir impounded by Challawa Gorge Dam. Constructed 1990-1992.</obo:IAO_0000115>
        <oboInOwl:hasOBONamespace>GAZ</oboInOwl:hasOBONamespace>
        <oboInOwl:id>GAZ:00233425</oboInOwl:id>
        <rdfs:label>Challawa Gorge Reservoir</rdfs:label>
    </owl:NamedIndividual>
    


    <!-- http://purl.obolibrary.org/obo/GAZ_00233427 -->

    <owl:NamedIndividual rdf:about="http://purl.obolibrary.org/obo/GAZ_00233427">
        <obo:IAO_0000115>A dam.</obo:IAO_0000115>
        <oboInOwl:hasOBONamespace>GAZ</oboInOwl:hasOBONamespace>
        <oboInOwl:id>GAZ:00233427</oboInOwl:id>
        <rdfs:label>Tiga Dam</rdfs:label>
    </owl:NamedIndividual>
    


    <!-- http://purl.obolibrary.org/obo/GAZ_00233432 -->

    <owl:NamedIndividual rdf:about="http://purl.obolibrary.org/obo/GAZ_00233432">
        <obo:RO_0001025 rdf:resource="http://purl.obolibrary.org/obo/GAZ_00051198"/>
        <obo:IAO_0000115>An oasis surrounded by the Tenere dessert and the dunes of the Erg of Bilma in eastern Niger, placed on the western edge of the small Agram mountain outcropping.</obo:IAO_0000115>
        <oboInOwl:hasOBONamespace>GAZ</oboInOwl:hasOBONamespace>
        <oboInOwl:id>GAZ:00233432</oboInOwl:id>
        <rdfs:label>Fachi</rdfs:label>
    </owl:NamedIndividual>
    


    <!-- http://purl.obolibrary.org/obo/GAZ_00233433 -->

    <owl:NamedIndividual rdf:about="http://purl.obolibrary.org/obo/GAZ_00233433">
        <obo:RO_0001025 rdf:resource="http://purl.obolibrary.org/obo/GAZ_00000826"/>
        <obo:IAO_0000115>Un affluent fossile du fleuve Niger et constitue le plus bas prolongement de la vallee du Tadiss (situee dans la region de Tahoua au Niger.</obo:IAO_0000115>
        <oboInOwl:hasOBONamespace>GAZ</oboInOwl:hasOBONamespace>
        <oboInOwl:id>GAZ:00233433</oboInOwl:id>
        <rdfs:label>Dallol Maouri</rdfs:label>
    </owl:NamedIndividual>
    


    <!-- http://purl.obolibrary.org/obo/GAZ_00233534 -->

    <owl:NamedIndividual rdf:about="http://purl.obolibrary.org/obo/GAZ_00233534">
        <obo:IAO_0000115>A lake. Formed by a widening of the channel of the Bahr el Ghazal.</obo:IAO_0000115>
        <oboInOwl:hasOBONamespace>GAZ</oboInOwl:hasOBONamespace>
        <oboInOwl:id>GAZ:00233534</oboInOwl:id>
        <rdfs:label>Lake Ambadi</rdfs:label>
    </owl:NamedIndividual>
    


    <!-- http://purl.obolibrary.org/obo/GAZ_00233536 -->

    <owl:NamedIndividual rdf:about="http://purl.obolibrary.org/obo/GAZ_00233536">
        <obo:IAO_0000115>A dam on the Blue Nile near the town of Sennar, Sudan. Constructed 1925.</obo:IAO_0000115>
        <oboInOwl:hasOBONamespace>GAZ</oboInOwl:hasOBONamespace>
        <oboInOwl:id>GAZ:00233536</oboInOwl:id>
        <rdfs:label>Sennar Dam</rdfs:label>
    </owl:NamedIndividual>
    


    <!-- http://purl.obolibrary.org/obo/GAZ_00233537 -->

    <owl:NamedIndividual rdf:about="http://purl.obolibrary.org/obo/GAZ_00233537">
        <obo:IAO_0000115>A hydroelectric dam. Impounds El Roseires Lake. Completed 1966.</obo:IAO_0000115>
        <oboInOwl:hasOBONamespace>GAZ</oboInOwl:hasOBONamespace>
        <oboInOwl:id>GAZ:00233537</oboInOwl:id>
        <rdfs:label>El Roseires Dam</rdfs:label>
    </owl:NamedIndividual>
    


    <!-- http://purl.obolibrary.org/obo/GAZ_00233540 -->

    <owl:NamedIndividual rdf:about="http://purl.obolibrary.org/obo/GAZ_00233540">
        <obo:IAO_0000115>An island on the White Nile to the south of Khartoum, Sudan.</obo:IAO_0000115>
        <oboInOwl:hasOBONamespace>GAZ</oboInOwl:hasOBONamespace>
        <oboInOwl:id>GAZ:00233540</oboInOwl:id>
        <rdfs:label>Aba Island</rdfs:label>
    </owl:NamedIndividual>
    


    <!-- http://purl.obolibrary.org/obo/GAZ_00233541 -->

    <owl:NamedIndividual rdf:about="http://purl.obolibrary.org/obo/GAZ_00233541">
        <obo:IAO_0000115>One of the biggest islands in the Nile and the second biggest island in Sudan. It is 56 km Northern to Dongola the capital of the Northern State in Sudan.</obo:IAO_0000115>
        <oboInOwl:hasOBONamespace>GAZ</oboInOwl:hasOBONamespace>
        <oboInOwl:id>GAZ:00233541</oboInOwl:id>
        <rdfs:label>Badien Island</rdfs:label>
    </owl:NamedIndividual>
    


    <!-- http://purl.obolibrary.org/obo/GAZ_00233542 -->

    <owl:NamedIndividual rdf:about="http://purl.obolibrary.org/obo/GAZ_00233542">
        <obo:IAO_0000115>A large island in the Nile River in Nubia between the second and third cataracts. It is 12 km long and 5.5 km wide.</obo:IAO_0000115>
        <oboInOwl:hasOBONamespace>GAZ</oboInOwl:hasOBONamespace>
        <oboInOwl:id>GAZ:00233542</oboInOwl:id>
        <rdfs:label>Sai</rdfs:label>
    </owl:NamedIndividual>
    


    <!-- http://purl.obolibrary.org/obo/GAZ_00233543 -->

    <owl:NamedIndividual rdf:about="http://purl.obolibrary.org/obo/GAZ_00233543">
        <obo:IAO_0000115>An island in Sudan where the White Nile and Blue Nile merge to form the main Nile. It is surrounded by Khartoum, Omdurman and Khartoum North.</obo:IAO_0000115>
        <oboInOwl:hasOBONamespace>GAZ</oboInOwl:hasOBONamespace>
        <oboInOwl:id>GAZ:00233543</oboInOwl:id>
        <rdfs:label>Tuti Island</rdfs:label>
    </owl:NamedIndividual>
    


    <!-- http://purl.obolibrary.org/obo/GAZ_00233583 -->

    <owl:NamedIndividual rdf:about="http://purl.obolibrary.org/obo/GAZ_00233583">
        <oboInOwl:hasOBONamespace>GAZ</oboInOwl:hasOBONamespace>
        <oboInOwl:id>GAZ:00233583</oboInOwl:id>
        <rdfs:label>Schott Dscherid</rdfs:label>
    </owl:NamedIndividual>
    


    <!-- http://purl.obolibrary.org/obo/GAZ_00234121 -->

    <owl:NamedIndividual rdf:about="http://purl.obolibrary.org/obo/GAZ_00234121">
        <obo:IAO_0000115>A river. It rises in the Mandaras, passing and swelling the Kebi in the North Province.</obo:IAO_0000115>
        <oboInOwl:hasOBONamespace>GAZ</oboInOwl:hasOBONamespace>
        <oboInOwl:id>GAZ:00234121</oboInOwl:id>
        <rdfs:label>Mayo Louti</rdfs:label>
    </owl:NamedIndividual>
    


    <!-- http://purl.obolibrary.org/obo/GAZ_00234122 -->

    <owl:NamedIndividual rdf:about="http://purl.obolibrary.org/obo/GAZ_00234122">
        <obo:IAO_0000115>A river that flows northwest from the Kalamaloue National Park and forms the northernmost stretch of the border between Cameroon and Nigeria.</obo:IAO_0000115>
        <oboInOwl:hasOBONamespace>GAZ</oboInOwl:hasOBONamespace>
        <oboInOwl:id>GAZ:00234122</oboInOwl:id>
        <rdfs:label>El Beid River</rdfs:label>
    </owl:NamedIndividual>
    


    <!-- http://purl.obolibrary.org/obo/GAZ_00234124 -->

    <owl:NamedIndividual rdf:about="http://purl.obolibrary.org/obo/GAZ_00234124">
        <obo:IAO_0000115>A river.</obo:IAO_0000115>
        <oboInOwl:hasOBONamespace>GAZ</oboInOwl:hasOBONamespace>
        <oboInOwl:id>GAZ:00234124</oboInOwl:id>
        <rdfs:label>Serbewel River</rdfs:label>
    </owl:NamedIndividual>
    


    <!-- http://purl.obolibrary.org/obo/GAZ_00237174 -->

    <owl:NamedIndividual rdf:about="http://purl.obolibrary.org/obo/GAZ_00237174">
        <obo:IAO_0000115>A hydroelectric power station across the White Nile near to its source at Lake Victoria in Uganda.</obo:IAO_0000115>
        <oboInOwl:hasOBONamespace>GAZ</oboInOwl:hasOBONamespace>
        <oboInOwl:id>GAZ:00237174</oboInOwl:id>
        <rdfs:label>Nalubaale Power Station</rdfs:label>
    </owl:NamedIndividual>
    


    <!-- http://purl.obolibrary.org/obo/GAZ_00237175 -->

    <owl:NamedIndividual rdf:about="http://purl.obolibrary.org/obo/GAZ_00237175">
        <obo:IAO_0000115>A hydroelectric power station located in Jinja, Jinja District, in eastern central Uganda.</obo:IAO_0000115>
        <oboInOwl:hasOBONamespace>GAZ</oboInOwl:hasOBONamespace>
        <oboInOwl:id>GAZ:00237175</oboInOwl:id>
        <rdfs:label>Kiira Power Station</rdfs:label>
    </owl:NamedIndividual>
    


    <!-- http://purl.obolibrary.org/obo/GAZ_00237176 -->

    <owl:NamedIndividual rdf:about="http://purl.obolibrary.org/obo/GAZ_00237176">
        <obo:IAO_0000115>A hydroelectric power project located at the headwaters of River Nile, about 16 km north of Jinja at the former location of Bujagali Falls.</obo:IAO_0000115>
        <oboInOwl:hasOBONamespace>GAZ</oboInOwl:hasOBONamespace>
        <oboInOwl:id>GAZ:00237176</oboInOwl:id>
        <rdfs:label>Bujagali Power Station</rdfs:label>
    </owl:NamedIndividual>
    


    <!-- http://purl.obolibrary.org/obo/GAZ_00237412 -->

    <owl:NamedIndividual rdf:about="http://purl.obolibrary.org/obo/GAZ_00237412">
        <obo:IAO_0000115>A river of eastern Uganda in eastern Africa. It flows in a southern and south-westerly direction and eventually via the Okere River reaches Lake Kyoga.</obo:IAO_0000115>
        <oboInOwl:hasOBONamespace>GAZ</oboInOwl:hasOBONamespace>
        <oboInOwl:id>GAZ:00237412</oboInOwl:id>
        <rdfs:label>Okot River</rdfs:label>
    </owl:NamedIndividual>
    


    <!-- http://purl.obolibrary.org/obo/GAZ_00242137 -->

    <owl:NamedIndividual rdf:about="http://purl.obolibrary.org/obo/GAZ_00242137">
        <obo:IAO_0000115>A river located in Anambra, a southeastern state in Nigeria. The river is the most important feeder of the River Niger below Lokoja.</obo:IAO_0000115>
        <oboInOwl:hasOBONamespace>GAZ</oboInOwl:hasOBONamespace>
        <oboInOwl:id>GAZ:00242137</oboInOwl:id>
        <rdfs:label>Anambra River</rdfs:label>
    </owl:NamedIndividual>
    


    <!-- http://purl.obolibrary.org/obo/GAZ_00242175 -->

    <owl:NamedIndividual rdf:about="http://purl.obolibrary.org/obo/GAZ_00242175">
        <obo:IAO_0000115>A distributary of the Niger Delta, in southern Nigeria.</obo:IAO_0000115>
        <oboInOwl:hasOBONamespace>GAZ</oboInOwl:hasOBONamespace>
        <oboInOwl:id>GAZ:00242175</oboInOwl:id>
        <rdfs:label>Forcados River</rdfs:label>
    </owl:NamedIndividual>
    


    <!-- http://purl.obolibrary.org/obo/GAZ_00242176 -->

    <owl:NamedIndividual rdf:about="http://purl.obolibrary.org/obo/GAZ_00242176">
        <obo:IAO_0000115>A distributary of the Niger Delta, in southern Nigeria.</obo:IAO_0000115>
        <oboInOwl:hasOBONamespace>GAZ</oboInOwl:hasOBONamespace>
        <oboInOwl:id>GAZ:00242176</oboInOwl:id>
        <rdfs:label>Nun River</rdfs:label>
    </owl:NamedIndividual>
    


    <!-- http://purl.obolibrary.org/obo/GAZ_00242177 -->

    <owl:NamedIndividual rdf:about="http://purl.obolibrary.org/obo/GAZ_00242177">
        <obo:IAO_0000115>A distributary of the Niger Delta, in southern Nigeria.</obo:IAO_0000115>
        <oboInOwl:hasOBONamespace>GAZ</oboInOwl:hasOBONamespace>
        <oboInOwl:id>GAZ:00242177</oboInOwl:id>
        <rdfs:label>Escravos River</rdfs:label>
    </owl:NamedIndividual>
    


    <!-- http://purl.obolibrary.org/obo/GAZ_00242187 -->

    <owl:NamedIndividual rdf:about="http://purl.obolibrary.org/obo/GAZ_00242187">
        <obo:IAO_0000115>A river. A tributary of the Katsina-Ala River.</obo:IAO_0000115>
        <oboInOwl:hasOBONamespace>GAZ</oboInOwl:hasOBONamespace>
        <oboInOwl:id>GAZ:00242187</oboInOwl:id>
        <rdfs:label>River Gamano</rdfs:label>
    </owl:NamedIndividual>
    


    <!-- http://purl.obolibrary.org/obo/GAZ_00242188 -->

    <owl:NamedIndividual rdf:about="http://purl.obolibrary.org/obo/GAZ_00242188">
        <obo:IAO_0000115>A dam. Impounds Kainji Lake. Constructed 1964-1968.</obo:IAO_0000115>
        <oboInOwl:hasOBONamespace>GAZ</oboInOwl:hasOBONamespace>
        <oboInOwl:id>GAZ:00242188</oboInOwl:id>
        <rdfs:label>Kainji Dam</rdfs:label>
    </owl:NamedIndividual>
    


    <!-- http://purl.obolibrary.org/obo/GAZ_00242205 -->

    <owl:NamedIndividual rdf:about="http://purl.obolibrary.org/obo/GAZ_00242205">
        <obo:IAO_0000115>A river in Nigeria that flows into Lake Chad and the Chad Basin.</obo:IAO_0000115>
        <oboInOwl:hasOBONamespace>GAZ</oboInOwl:hasOBONamespace>
        <oboInOwl:id>GAZ:00242205</oboInOwl:id>
        <rdfs:label>Ngadda River</rdfs:label>
    </owl:NamedIndividual>
    


    <!-- http://purl.obolibrary.org/obo/GAZ_00242206 -->

    <owl:NamedIndividual rdf:about="http://purl.obolibrary.org/obo/GAZ_00242206">
        <obo:RO_0001025 rdf:resource="http://purl.obolibrary.org/obo/GAZ_00242205"/>
        <obo:IAO_0000115>A dam.</obo:IAO_0000115>
        <oboInOwl:hasOBONamespace>GAZ</oboInOwl:hasOBONamespace>
        <oboInOwl:id>GAZ:00242206</oboInOwl:id>
        <rdfs:label>Alau Dam</rdfs:label>
    </owl:NamedIndividual>
    


    <!-- http://purl.obolibrary.org/obo/GAZ_00246604 -->

    <owl:NamedIndividual rdf:about="http://purl.obolibrary.org/obo/GAZ_00246604">
        <obo:IAO_0000115>A freshwater lake. One of the most isolated occurrences of free surface water in the Sahara. It is situated near the southwestern extremity of the plateau, Adrar Nahalet, which extends westwards from the massif of the A&apos;Haggar. The permanent guelta (pool), 13 m wide when full and 6 m deep, is inside a volcanic crater which partly encloses a valley. It collects water from two oueds which drain Ziza Mountain, to the south, and is reputed to have no underground input. Several small temporary pools also occur in the bed of the main oued draining Mount Ziza.</obo:IAO_0000115>
        <oboInOwl:hasOBONamespace>GAZ</oboInOwl:hasOBONamespace>
        <oboInOwl:id>GAZ:00246604</oboInOwl:id>
        <rdfs:label>Gueltas of Ziza</rdfs:label>
    </owl:NamedIndividual>
    


    <!-- http://purl.obolibrary.org/obo/GAZ_00246788 -->

    <owl:NamedIndividual rdf:about="http://purl.obolibrary.org/obo/GAZ_00246788">
        <obo:IAO_0000115>A river.</obo:IAO_0000115>
        <oboInOwl:hasOBONamespace>GAZ</oboInOwl:hasOBONamespace>
        <oboInOwl:id>GAZ:00246788</oboInOwl:id>
        <rdfs:label>Kompa Gorau River</rdfs:label>
    </owl:NamedIndividual>
    


    <!-- http://purl.obolibrary.org/obo/GAZ_00247034 -->

    <owl:NamedIndividual rdf:about="http://purl.obolibrary.org/obo/GAZ_00247034">
        <obo:IAO_0000115>A dam.</obo:IAO_0000115>
        <oboInOwl:hasOBONamespace>GAZ</oboInOwl:hasOBONamespace>
        <oboInOwl:id>GAZ:00247034</oboInOwl:id>
        <rdfs:label>Tougouri Barrage</rdfs:label>
    </owl:NamedIndividual>
    


    <!-- http://purl.obolibrary.org/obo/GAZ_00247035 -->

    <owl:NamedIndividual rdf:about="http://purl.obolibrary.org/obo/GAZ_00247035">
        <obo:IAO_0000115>A dam.</obo:IAO_0000115>
        <oboInOwl:hasOBONamespace>GAZ</oboInOwl:hasOBONamespace>
        <oboInOwl:id>GAZ:00247035</oboInOwl:id>
        <rdfs:label>Yalogo Barrage</rdfs:label>
    </owl:NamedIndividual>
    


    <!-- http://purl.obolibrary.org/obo/GAZ_00247169 -->

    <owl:NamedIndividual rdf:about="http://purl.obolibrary.org/obo/GAZ_00247169">
        <obo:IAO_0000115>A river.</obo:IAO_0000115>
        <oboInOwl:hasOBONamespace>GAZ</oboInOwl:hasOBONamespace>
        <oboInOwl:id>GAZ:00247169</oboInOwl:id>
        <rdfs:label>Bangoran River</rdfs:label>
    </owl:NamedIndividual>
    


    <!-- http://purl.obolibrary.org/obo/GAZ_00247178 -->

    <owl:NamedIndividual rdf:about="http://purl.obolibrary.org/obo/GAZ_00247178">
        <obo:IAO_0000115>A depression.</obo:IAO_0000115>
        <oboInOwl:hasOBONamespace>GAZ</oboInOwl:hasOBONamespace>
        <oboInOwl:id>GAZ:00247178</oboInOwl:id>
        <rdfs:label>Depression du Mourdi</rdfs:label>
    </owl:NamedIndividual>
    


    <!-- http://purl.obolibrary.org/obo/GAZ_00247180 -->

    <owl:NamedIndividual rdf:about="http://purl.obolibrary.org/obo/GAZ_00247180">
        <obo:IAO_0000115>A mountain range.</obo:IAO_0000115>
        <oboInOwl:hasOBONamespace>GAZ</oboInOwl:hasOBONamespace>
        <oboInOwl:id>GAZ:00247180</oboInOwl:id>
        <rdfs:label>Massif du Kerkour Nourene</rdfs:label>
    </owl:NamedIndividual>
    


    <!-- http://purl.obolibrary.org/obo/GAZ_00247191 -->

    <owl:NamedIndividual rdf:about="http://purl.obolibrary.org/obo/GAZ_00247191">
        <obo:IAO_0000115>A lake. Located on the Mayo Kebbi.</obo:IAO_0000115>
        <oboInOwl:hasOBONamespace>GAZ</oboInOwl:hasOBONamespace>
        <oboInOwl:id>GAZ:00247191</oboInOwl:id>
        <rdfs:label>Lake Tikem</rdfs:label>
    </owl:NamedIndividual>
    


    <!-- http://purl.obolibrary.org/obo/GAZ_00247192 -->

    <owl:NamedIndividual rdf:about="http://purl.obolibrary.org/obo/GAZ_00247192">
        <obo:IAO_0000115>A lake. Located on the Mayo Kebbi.</obo:IAO_0000115>
        <oboInOwl:hasOBONamespace>GAZ</oboInOwl:hasOBONamespace>
        <oboInOwl:id>GAZ:00247192</oboInOwl:id>
        <rdfs:label>Lake N&apos;Gara</rdfs:label>
    </owl:NamedIndividual>
    


    <!-- http://purl.obolibrary.org/obo/GAZ_00247193 -->

    <owl:NamedIndividual rdf:about="http://purl.obolibrary.org/obo/GAZ_00247193">
        <obo:RO_0001025 rdf:resource="http://purl.obolibrary.org/obo/GAZ_00230256"/>
        <obo:IAO_0000115>A lake.</obo:IAO_0000115>
        <oboInOwl:hasOBONamespace>GAZ</oboInOwl:hasOBONamespace>
        <oboInOwl:id>GAZ:00247193</oboInOwl:id>
        <rdfs:label>Lake Trene</rdfs:label>
    </owl:NamedIndividual>
    


    <!-- http://purl.obolibrary.org/obo/GAZ_00247194 -->

    <owl:NamedIndividual rdf:about="http://purl.obolibrary.org/obo/GAZ_00247194">
        <obo:IAO_0000115>Aa ridge crosses the middle of Lake Chad from east to west. Although in the `normal&apos; lake this is inundated, it restricts circulation. Thus the northern part of the lake is significantly more saline than the southern half.</obo:IAO_0000115>
        <oboInOwl:hasOBONamespace>GAZ</oboInOwl:hasOBONamespace>
        <oboInOwl:id>GAZ:00247194</oboInOwl:id>
        <rdfs:label>Grande Barriere</rdfs:label>
    </owl:NamedIndividual>
    


    <!-- http://purl.obolibrary.org/obo/GAZ_00247215 -->

    <owl:NamedIndividual rdf:about="http://purl.obolibrary.org/obo/GAZ_00247215">
        <obo:RO_0001025 rdf:resource="http://purl.obolibrary.org/obo/GAZ_00230256"/>
        <oboInOwl:hasOBONamespace>GAZ</oboInOwl:hasOBONamespace>
        <oboInOwl:id>GAZ:00247215</oboInOwl:id>
        <rdfs:label>Lake Lere</rdfs:label>
    </owl:NamedIndividual>
    


    <!-- http://purl.obolibrary.org/obo/GAZ_00247676 -->

    <owl:NamedIndividual rdf:about="http://purl.obolibrary.org/obo/GAZ_00247676">
        <obo:IAO_0000115>An intermittent river in the Sahara.</obo:IAO_0000115>
        <oboInOwl:hasOBONamespace>GAZ</oboInOwl:hasOBONamespace>
        <oboInOwl:id>GAZ:00247676</oboInOwl:id>
        <rdfs:label>Oued Saoura</rdfs:label>
    </owl:NamedIndividual>
    


    <!-- http://purl.obolibrary.org/obo/GAZ_00247997 -->

    <owl:NamedIndividual rdf:about="http://purl.obolibrary.org/obo/GAZ_00247997">
        <obo:RO_0001025 rdf:resource="http://purl.obolibrary.org/obo/GAZ_00009949"/>
        <obo:IAO_0000115>A lake.</obo:IAO_0000115>
        <oboInOwl:hasOBONamespace>GAZ</oboInOwl:hasOBONamespace>
        <oboInOwl:id>GAZ:00247997</oboInOwl:id>
        <rdfs:label>Birkat al Mallah</rdfs:label>
    </owl:NamedIndividual>
    


    <!-- http://purl.obolibrary.org/obo/GAZ_00247998 -->

    <owl:NamedIndividual rdf:about="http://purl.obolibrary.org/obo/GAZ_00247998">
        <obo:RO_0001025 rdf:resource="http://purl.obolibrary.org/obo/GAZ_00009949"/>
        <obo:IAO_0000115>A lake.</obo:IAO_0000115>
        <oboInOwl:hasOBONamespace>GAZ</oboInOwl:hasOBONamespace>
        <oboInOwl:id>GAZ:00247998</oboInOwl:id>
        <rdfs:label>Birkat al Qatta</rdfs:label>
    </owl:NamedIndividual>
    


    <!-- http://purl.obolibrary.org/obo/GAZ_00247999 -->

    <owl:NamedIndividual rdf:about="http://purl.obolibrary.org/obo/GAZ_00247999">
        <obo:RO_0001025 rdf:resource="http://purl.obolibrary.org/obo/GAZ_00009949"/>
        <obo:IAO_0000115>A lake.</obo:IAO_0000115>
        <oboInOwl:hasOBONamespace>GAZ</oboInOwl:hasOBONamespace>
        <oboInOwl:id>GAZ:00247999</oboInOwl:id>
        <rdfs:label>Lake Faraontya</rdfs:label>
    </owl:NamedIndividual>
    


    <!-- http://purl.obolibrary.org/obo/GAZ_00248000 -->

    <owl:NamedIndividual rdf:about="http://purl.obolibrary.org/obo/GAZ_00248000">
        <obo:RO_0001025 rdf:resource="http://purl.obolibrary.org/obo/GAZ_00009949"/>
        <obo:IAO_0000115>A coastal lagoon.</obo:IAO_0000115>
        <oboInOwl:hasOBONamespace>GAZ</oboInOwl:hasOBONamespace>
        <oboInOwl:id>GAZ:00248000</oboInOwl:id>
        <rdfs:label>Buhayrat al Manzilah</rdfs:label>
    </owl:NamedIndividual>
    


    <!-- http://purl.obolibrary.org/obo/GAZ_00248001 -->

    <owl:NamedIndividual rdf:about="http://purl.obolibrary.org/obo/GAZ_00248001">
        <obo:RO_0001025 rdf:resource="http://purl.obolibrary.org/obo/GAZ_00009949"/>
        <obo:IAO_0000115>A lake.</obo:IAO_0000115>
        <oboInOwl:hasOBONamespace>GAZ</oboInOwl:hasOBONamespace>
        <oboInOwl:id>GAZ:00248001</oboInOwl:id>
        <rdfs:label>Birkat Muhayshir</rdfs:label>
    </owl:NamedIndividual>
    


    <!-- http://purl.obolibrary.org/obo/GAZ_00248009 -->

    <owl:NamedIndividual rdf:about="http://purl.obolibrary.org/obo/GAZ_00248009">
        <obo:RO_0001025 rdf:resource="http://purl.obolibrary.org/obo/GAZ_00051197"/>
        <obo:IAO_0000115>A depression, about 25 m below sea level at its deepest. Bounded by steep slopes on the northern side, reaching about 120-160 m asl, but by much gentler slopes to the south and southeast.</obo:IAO_0000115>
        <oboInOwl:hasOBONamespace>GAZ</oboInOwl:hasOBONamespace>
        <oboInOwl:id>GAZ:00248009</oboInOwl:id>
        <rdfs:label>Siwa Depression</rdfs:label>
    </owl:NamedIndividual>
    


    <!-- http://purl.obolibrary.org/obo/GAZ_00248010 -->

    <owl:NamedIndividual rdf:about="http://purl.obolibrary.org/obo/GAZ_00248010">
        <obo:RO_0001025 rdf:resource="http://purl.obolibrary.org/obo/GAZ_00248009"/>
        <obo:IAO_0000115>An oasis.</obo:IAO_0000115>
        <oboInOwl:hasOBONamespace>GAZ</oboInOwl:hasOBONamespace>
        <oboInOwl:id>GAZ:00248010</oboInOwl:id>
        <rdfs:label>Shiyata</rdfs:label>
    </owl:NamedIndividual>
    


    <!-- http://purl.obolibrary.org/obo/GAZ_00248011 -->

    <owl:NamedIndividual rdf:about="http://purl.obolibrary.org/obo/GAZ_00248011">
        <obo:RO_0001025 rdf:resource="http://purl.obolibrary.org/obo/GAZ_00248009"/>
        <obo:IAO_0000115>A saline lake.</obo:IAO_0000115>
        <oboInOwl:hasOBONamespace>GAZ</oboInOwl:hasOBONamespace>
        <oboInOwl:id>GAZ:00248011</oboInOwl:id>
        <rdfs:label>Birkat al Maraqi</rdfs:label>
    </owl:NamedIndividual>
    


    <!-- http://purl.obolibrary.org/obo/GAZ_00248012 -->

    <owl:NamedIndividual rdf:about="http://purl.obolibrary.org/obo/GAZ_00248012">
        <obo:RO_0001025 rdf:resource="http://purl.obolibrary.org/obo/GAZ_00248009"/>
        <obo:IAO_0000115>A saline lake.</obo:IAO_0000115>
        <oboInOwl:hasOBONamespace>GAZ</oboInOwl:hasOBONamespace>
        <oboInOwl:id>GAZ:00248012</oboInOwl:id>
        <rdfs:label>Birkat el Zaytun</rdfs:label>
    </owl:NamedIndividual>
    


    <!-- http://purl.obolibrary.org/obo/GAZ_00248013 -->

    <owl:NamedIndividual rdf:about="http://purl.obolibrary.org/obo/GAZ_00248013">
        <obo:RO_0001025 rdf:resource="http://purl.obolibrary.org/obo/GAZ_00248009"/>
        <obo:IAO_0000115>A saline lake.</obo:IAO_0000115>
        <oboInOwl:hasOBONamespace>GAZ</oboInOwl:hasOBONamespace>
        <oboInOwl:id>GAZ:00248013</oboInOwl:id>
        <rdfs:label>Birkat Siwah</rdfs:label>
    </owl:NamedIndividual>
    


    <!-- http://purl.obolibrary.org/obo/GAZ_00248014 -->

    <owl:NamedIndividual rdf:about="http://purl.obolibrary.org/obo/GAZ_00248014">
        <obo:RO_0001025 rdf:resource="http://purl.obolibrary.org/obo/GAZ_00248009"/>
        <obo:IAO_0000115>A saline lake.</obo:IAO_0000115>
        <oboInOwl:hasOBONamespace>GAZ</oboInOwl:hasOBONamespace>
        <oboInOwl:id>GAZ:00248014</oboInOwl:id>
        <rdfs:label>Birkat Aghurmi</rdfs:label>
    </owl:NamedIndividual>
    


    <!-- http://purl.obolibrary.org/obo/GAZ_00248015 -->

    <owl:NamedIndividual rdf:about="http://purl.obolibrary.org/obo/GAZ_00248015">
        <obo:RO_0001025 rdf:resource="http://purl.obolibrary.org/obo/GAZ_00248009"/>
        <obo:IAO_0000115>A saline lake.</obo:IAO_0000115>
        <oboInOwl:hasOBONamespace>GAZ</oboInOwl:hasOBONamespace>
        <oboInOwl:id>GAZ:00248015</oboInOwl:id>
        <rdfs:label>Birkat Samar Abu Ishaq</rdfs:label>
    </owl:NamedIndividual>
    


    <!-- http://purl.obolibrary.org/obo/GAZ_00248016 -->

    <owl:NamedIndividual rdf:about="http://purl.obolibrary.org/obo/GAZ_00248016">
        <obo:RO_0001025 rdf:resource="http://purl.obolibrary.org/obo/GAZ_00051196"/>
        <obo:IAO_0000115>A semi-permanent saline lake.</obo:IAO_0000115>
        <oboInOwl:hasOBONamespace>GAZ</oboInOwl:hasOBONamespace>
        <oboInOwl:id>GAZ:00248016</oboInOwl:id>
        <rdfs:label>Lake Sitra</rdfs:label>
    </owl:NamedIndividual>
    


    <!-- http://purl.obolibrary.org/obo/GAZ_00248017 -->

    <owl:NamedIndividual rdf:about="http://purl.obolibrary.org/obo/GAZ_00248017">
        <obo:RO_0001025 rdf:resource="http://purl.obolibrary.org/obo/GAZ_00051196"/>
        <obo:IAO_0000115>A semi-permanent saline lake.</obo:IAO_0000115>
        <oboInOwl:hasOBONamespace>GAZ</oboInOwl:hasOBONamespace>
        <oboInOwl:id>GAZ:00248017</oboInOwl:id>
        <rdfs:label>Lake el Bahrein</rdfs:label>
    </owl:NamedIndividual>
    


    <!-- http://purl.obolibrary.org/obo/GAZ_00248018 -->

    <owl:NamedIndividual rdf:about="http://purl.obolibrary.org/obo/GAZ_00248018">
        <obo:RO_0001025 rdf:resource="http://purl.obolibrary.org/obo/GAZ_00051196"/>
        <obo:IAO_0000115>A semi-permanent saline lake.</obo:IAO_0000115>
        <oboInOwl:hasOBONamespace>GAZ</oboInOwl:hasOBONamespace>
        <oboInOwl:id>GAZ:00248018</oboInOwl:id>
        <rdfs:label>Lake el Maghra</rdfs:label>
    </owl:NamedIndividual>
    


    <!-- http://purl.obolibrary.org/obo/GAZ_00248580 -->

    <owl:NamedIndividual rdf:about="http://purl.obolibrary.org/obo/GAZ_00248580">
        <obo:IAO_0000115>A river.</obo:IAO_0000115>
        <oboInOwl:hasOBONamespace>GAZ</oboInOwl:hasOBONamespace>
        <oboInOwl:id>GAZ:00248580</oboInOwl:id>
        <rdfs:label>Kourd River</rdfs:label>
    </owl:NamedIndividual>
    


    <!-- http://purl.obolibrary.org/obo/GAZ_00248581 -->

    <owl:NamedIndividual rdf:about="http://purl.obolibrary.org/obo/GAZ_00248581">
        <obo:IAO_0000115>A river.</obo:IAO_0000115>
        <oboInOwl:hasOBONamespace>GAZ</oboInOwl:hasOBONamespace>
        <oboInOwl:id>GAZ:00248581</oboInOwl:id>
        <rdfs:label>Yeremou River</rdfs:label>
    </owl:NamedIndividual>
    


    <!-- http://purl.obolibrary.org/obo/GAZ_00251838 -->

    <owl:NamedIndividual rdf:about="http://purl.obolibrary.org/obo/GAZ_00251838">
        <obo:IAO_0000115>An erg.</obo:IAO_0000115>
        <oboInOwl:hasOBONamespace>GAZ</oboInOwl:hasOBONamespace>
        <oboInOwl:id>GAZ:00251838</oboInOwl:id>
        <rdfs:label>Idhan Ubari</rdfs:label>
    </owl:NamedIndividual>
    


    <!-- http://purl.obolibrary.org/obo/GAZ_00252160 -->

    <owl:NamedIndividual rdf:about="http://purl.obolibrary.org/obo/GAZ_00252160">
        <obo:RO_0001025 rdf:resource="http://purl.obolibrary.org/obo/GAZ_00147864"/>
        <obo:IAO_0000115>A lake.</obo:IAO_0000115>
        <oboInOwl:hasOBONamespace>GAZ</oboInOwl:hasOBONamespace>
        <oboInOwl:id>GAZ:00252160</oboInOwl:id>
        <rdfs:label>Lac Korienze</rdfs:label>
    </owl:NamedIndividual>
    


    <!-- http://purl.obolibrary.org/obo/GAZ_00252163 -->

    <owl:NamedIndividual rdf:about="http://purl.obolibrary.org/obo/GAZ_00252163">
        <obo:IAO_0000115>A drainage canal.</obo:IAO_0000115>
        <oboInOwl:hasOBONamespace>GAZ</oboInOwl:hasOBONamespace>
        <oboInOwl:id>GAZ:00252163</oboInOwl:id>
        <rdfs:label>Canal du Sahel</rdfs:label>
    </owl:NamedIndividual>
    


    <!-- http://purl.obolibrary.org/obo/GAZ_00252194 -->

    <owl:NamedIndividual rdf:about="http://purl.obolibrary.org/obo/GAZ_00252194">
        <obo:RO_0001025 rdf:resource="http://purl.obolibrary.org/obo/GAZ_00252195"/>
        <obo:IAO_0000115>A guelta system.</obo:IAO_0000115>
        <oboInOwl:hasOBONamespace>GAZ</oboInOwl:hasOBONamespace>
        <oboInOwl:id>GAZ:00252194</oboInOwl:id>
        <rdfs:label>Gamra Ouarbi Gueltas</rdfs:label>
    </owl:NamedIndividual>
    


    <!-- http://purl.obolibrary.org/obo/GAZ_00252195 -->

    <owl:NamedIndividual rdf:about="http://purl.obolibrary.org/obo/GAZ_00252195">
        <obo:RO_0001025 rdf:resource="http://purl.obolibrary.org/obo/GAZ_00231580"/>
        <obo:IAO_0000115>A wadi.</obo:IAO_0000115>
        <oboInOwl:hasOBONamespace>GAZ</oboInOwl:hasOBONamespace>
        <oboInOwl:id>GAZ:00252195</oboInOwl:id>
        <rdfs:label>Oued Bourraga</rdfs:label>
    </owl:NamedIndividual>
    


    <!-- http://purl.obolibrary.org/obo/GAZ_00252196 -->

    <owl:NamedIndividual rdf:about="http://purl.obolibrary.org/obo/GAZ_00252196">
        <obo:RO_0001025 rdf:resource="http://purl.obolibrary.org/obo/GAZ_00252195"/>
        <obo:IAO_0000115>A spring.</obo:IAO_0000115>
        <oboInOwl:hasOBONamespace>GAZ</oboInOwl:hasOBONamespace>
        <oboInOwl:id>GAZ:00252196</oboInOwl:id>
        <rdfs:label>El Housseiniya</rdfs:label>
    </owl:NamedIndividual>
    


    <!-- http://purl.obolibrary.org/obo/GAZ_00252197 -->

    <owl:NamedIndividual rdf:about="http://purl.obolibrary.org/obo/GAZ_00252197">
        <obo:RO_0001025 rdf:resource="http://purl.obolibrary.org/obo/GAZ_00231580"/>
        <obo:IAO_0000115>An oasis. Located in the escarpment of the Tagant Plateau, in its southwestern extension towards Kiffa.</obo:IAO_0000115>
        <oboInOwl:hasOBONamespace>GAZ</oboInOwl:hasOBONamespace>
        <oboInOwl:id>GAZ:00252197</oboInOwl:id>
        <rdfs:label>Tartega Gueltas</rdfs:label>
    </owl:NamedIndividual>
    


    <!-- http://purl.obolibrary.org/obo/GAZ_00253017 -->

    <owl:NamedIndividual rdf:about="http://purl.obolibrary.org/obo/GAZ_00253017">
        <obo:RO_0001025 rdf:resource="http://purl.obolibrary.org/obo/GAZ_00000822"/>
        <obo:RO_0001025 rdf:resource="http://purl.obolibrary.org/obo/GAZ_00103898"/>
        <obo:IAO_0000115>A wadi.</obo:IAO_0000115>
        <oboInOwl:hasOBONamespace>GAZ</oboInOwl:hasOBONamespace>
        <oboInOwl:id>GAZ:00253017</oboInOwl:id>
        <rdfs:label>Ighalabelabene</rdfs:label>
    </owl:NamedIndividual>
    


    <!-- http://purl.obolibrary.org/obo/GAZ_00253018 -->

    <owl:NamedIndividual rdf:about="http://purl.obolibrary.org/obo/GAZ_00253018">
        <obo:RO_0001025 rdf:resource="http://purl.obolibrary.org/obo/GAZ_00000822"/>
        <obo:RO_0001025 rdf:resource="http://purl.obolibrary.org/obo/GAZ_00103898"/>
        <obo:IAO_0000115>A wadi.</obo:IAO_0000115>
        <oboInOwl:hasOBONamespace>GAZ</oboInOwl:hasOBONamespace>
        <oboInOwl:id>GAZ:00253018</oboInOwl:id>
        <rdfs:label>Nabarou</rdfs:label>
    </owl:NamedIndividual>
    


    <!-- http://purl.obolibrary.org/obo/GAZ_00253019 -->

    <owl:NamedIndividual rdf:about="http://purl.obolibrary.org/obo/GAZ_00253019">
        <obo:RO_0001025 rdf:resource="http://purl.obolibrary.org/obo/GAZ_00000822"/>
        <obo:RO_0001025 rdf:resource="http://purl.obolibrary.org/obo/GAZ_00103898"/>
        <obo:IAO_0000115>A wadi.</obo:IAO_0000115>
        <oboInOwl:hasOBONamespace>GAZ</oboInOwl:hasOBONamespace>
        <oboInOwl:id>GAZ:00253019</oboInOwl:id>
        <rdfs:label>Bagzane-n-Ammas</rdfs:label>
    </owl:NamedIndividual>
    


    <!-- http://purl.obolibrary.org/obo/GAZ_00253020 -->

    <owl:NamedIndividual rdf:about="http://purl.obolibrary.org/obo/GAZ_00253020">
        <obo:RO_0001025 rdf:resource="http://purl.obolibrary.org/obo/GAZ_00000822"/>
        <obo:RO_0001025 rdf:resource="http://purl.obolibrary.org/obo/GAZ_00103898"/>
        <obo:IAO_0000115>An intermittent river.</obo:IAO_0000115>
        <oboInOwl:hasOBONamespace>GAZ</oboInOwl:hasOBONamespace>
        <oboInOwl:id>GAZ:00253020</oboInOwl:id>
        <rdfs:label>Timia</rdfs:label>
    </owl:NamedIndividual>
    


    <!-- http://purl.obolibrary.org/obo/GAZ_00253021 -->

    <owl:NamedIndividual rdf:about="http://purl.obolibrary.org/obo/GAZ_00253021">
        <obo:RO_0001025 rdf:resource="http://purl.obolibrary.org/obo/GAZ_00000822"/>
        <obo:RO_0001025 rdf:resource="http://purl.obolibrary.org/obo/GAZ_00103898"/>
        <obo:IAO_0000115>A wadi.</obo:IAO_0000115>
        <oboInOwl:hasOBONamespace>GAZ</oboInOwl:hasOBONamespace>
        <oboInOwl:id>GAZ:00253021</oboInOwl:id>
        <rdfs:label>Tamgak</rdfs:label>
    </owl:NamedIndividual>
    


    <!-- http://purl.obolibrary.org/obo/GAZ_00253022 -->

    <owl:NamedIndividual rdf:about="http://purl.obolibrary.org/obo/GAZ_00253022">
        <obo:RO_0001025 rdf:resource="http://purl.obolibrary.org/obo/GAZ_00000822"/>
        <obo:RO_0001025 rdf:resource="http://purl.obolibrary.org/obo/GAZ_00103898"/>
        <obo:IAO_0000115>A plateau.</obo:IAO_0000115>
        <oboInOwl:hasOBONamespace>GAZ</oboInOwl:hasOBONamespace>
        <oboInOwl:id>GAZ:00253022</oboInOwl:id>
        <rdfs:label>Djado Massif</rdfs:label>
    </owl:NamedIndividual>
    


    <!-- http://purl.obolibrary.org/obo/GAZ_00253023 -->

    <owl:NamedIndividual rdf:about="http://purl.obolibrary.org/obo/GAZ_00253023">
        <obo:RO_0001025 rdf:resource="http://purl.obolibrary.org/obo/GAZ_00000822"/>
        <obo:RO_0001025 rdf:resource="http://purl.obolibrary.org/obo/GAZ_00103898"/>
        <obo:IAO_0000115>A plateau.</obo:IAO_0000115>
        <oboInOwl:hasOBONamespace>GAZ</oboInOwl:hasOBONamespace>
        <oboInOwl:id>GAZ:00253023</oboInOwl:id>
        <rdfs:label>Kaquar Massif</rdfs:label>
    </owl:NamedIndividual>
    


    <!-- http://purl.obolibrary.org/obo/GAZ_00253024 -->

    <owl:NamedIndividual rdf:about="http://purl.obolibrary.org/obo/GAZ_00253024">
        <obo:RO_0001025 rdf:resource="http://purl.obolibrary.org/obo/GAZ_00000822"/>
        <obo:RO_0001025 rdf:resource="http://purl.obolibrary.org/obo/GAZ_00103898"/>
        <obo:IAO_0000115>An escarpment.</obo:IAO_0000115>
        <oboInOwl:hasOBONamespace>GAZ</oboInOwl:hasOBONamespace>
        <oboInOwl:id>GAZ:00253024</oboInOwl:id>
        <rdfs:label>Fachi Massif</rdfs:label>
    </owl:NamedIndividual>
    


    <!-- http://purl.obolibrary.org/obo/GAZ_00253029 -->

    <owl:NamedIndividual rdf:about="http://purl.obolibrary.org/obo/GAZ_00253029">
        <obo:IAO_0000115>A river.</obo:IAO_0000115>
        <oboInOwl:hasOBONamespace>GAZ</oboInOwl:hasOBONamespace>
        <oboInOwl:id>GAZ:00253029</oboInOwl:id>
        <rdfs:label>Sambreiro River</rdfs:label>
    </owl:NamedIndividual>
    


    <!-- http://purl.obolibrary.org/obo/GAZ_00253030 -->

    <owl:NamedIndividual rdf:about="http://purl.obolibrary.org/obo/GAZ_00253030">
        <obo:IAO_0000115>A river.</obo:IAO_0000115>
        <oboInOwl:hasOBONamespace>GAZ</oboInOwl:hasOBONamespace>
        <oboInOwl:id>GAZ:00253030</oboInOwl:id>
        <rdfs:label>Bonny River</rdfs:label>
    </owl:NamedIndividual>
    


    <!-- http://purl.obolibrary.org/obo/GAZ_00253031 -->

    <owl:NamedIndividual rdf:about="http://purl.obolibrary.org/obo/GAZ_00253031">
        <obo:IAO_0000115>A river.</obo:IAO_0000115>
        <oboInOwl:hasOBONamespace>GAZ</oboInOwl:hasOBONamespace>
        <oboInOwl:id>GAZ:00253031</oboInOwl:id>
        <rdfs:label>Brass River</rdfs:label>
    </owl:NamedIndividual>
    


    <!-- http://purl.obolibrary.org/obo/GAZ_00256465 -->

    <owl:NamedIndividual rdf:about="http://purl.obolibrary.org/obo/GAZ_00256465">
        <obo:IAO_0000115>A river.</obo:IAO_0000115>
        <oboInOwl:hasOBONamespace>GAZ</oboInOwl:hasOBONamespace>
        <oboInOwl:id>GAZ:00256465</oboInOwl:id>
        <rdfs:label>Lileboak River</rdfs:label>
    </owl:NamedIndividual>
    


    <!-- http://purl.obolibrary.org/obo/GAZ_00256472 -->

    <owl:NamedIndividual rdf:about="http://purl.obolibrary.org/obo/GAZ_00256472">
        <obo:IAO_0000115>A dam.</obo:IAO_0000115>
        <oboInOwl:hasOBONamespace>GAZ</oboInOwl:hasOBONamespace>
        <oboInOwl:id>GAZ:00256472</oboInOwl:id>
        <rdfs:label>Jebel Auliya Dam</rdfs:label>
    </owl:NamedIndividual>
    


    <!-- http://purl.obolibrary.org/obo/GAZ_00256473 -->

    <owl:NamedIndividual rdf:about="http://purl.obolibrary.org/obo/GAZ_00256473">
        <obo:IAO_0000115>A reservoir. Impounded by Jebel Auliya Dam.</obo:IAO_0000115>
        <oboInOwl:hasOBONamespace>GAZ</oboInOwl:hasOBONamespace>
        <oboInOwl:id>GAZ:00256473</oboInOwl:id>
        <rdfs:label>Jebel Auliya Reservoir</rdfs:label>
    </owl:NamedIndividual>
    


    <!-- http://purl.obolibrary.org/obo/GAZ_00256482 -->

    <owl:NamedIndividual rdf:about="http://purl.obolibrary.org/obo/GAZ_00256482">
        <obo:IAO_0000115>An artificial lake. Impounded by El Roseires Dam.</obo:IAO_0000115>
        <oboInOwl:hasOBONamespace>GAZ</oboInOwl:hasOBONamespace>
        <oboInOwl:id>GAZ:00256482</oboInOwl:id>
        <rdfs:label>El Roseires Lake</rdfs:label>
    </owl:NamedIndividual>
    


    <!-- http://purl.obolibrary.org/obo/GAZ_00256483 -->

    <owl:NamedIndividual rdf:about="http://purl.obolibrary.org/obo/GAZ_00256483">
        <obo:IAO_0000115>An artifiical lake. Impounded by Sennar Dam.</obo:IAO_0000115>
        <oboInOwl:hasOBONamespace>GAZ</oboInOwl:hasOBONamespace>
        <oboInOwl:id>GAZ:00256483</oboInOwl:id>
        <rdfs:label>Sennar Lake</rdfs:label>
    </owl:NamedIndividual>
    


    <!-- http://purl.obolibrary.org/obo/GAZ_00256484 -->

    <owl:NamedIndividual rdf:about="http://purl.obolibrary.org/obo/GAZ_00256484">
        <obo:IAO_0000115>A dam. Impounds Kashim el Girlba Lake. Completed 1964.</obo:IAO_0000115>
        <oboInOwl:hasOBONamespace>GAZ</oboInOwl:hasOBONamespace>
        <oboInOwl:id>GAZ:00256484</oboInOwl:id>
        <rdfs:label>Kashim el Girlba Dam</rdfs:label>
    </owl:NamedIndividual>
    


    <!-- http://purl.obolibrary.org/obo/GAZ_00256485 -->

    <owl:NamedIndividual rdf:about="http://purl.obolibrary.org/obo/GAZ_00256485">
        <obo:IAO_0000115>An artifiical lake. Impounded by Kashim el Girlba Dam. Completed 1964.</obo:IAO_0000115>
        <oboInOwl:hasOBONamespace>GAZ</oboInOwl:hasOBONamespace>
        <oboInOwl:id>GAZ:00256485</oboInOwl:id>
        <rdfs:label>Kashim el Girlba Lake</rdfs:label>
    </owl:NamedIndividual>
    


    <!-- http://purl.obolibrary.org/obo/GAZ_00256486 -->

    <owl:NamedIndividual rdf:about="http://purl.obolibrary.org/obo/GAZ_00256486">
        <rdf:type rdf:resource="http://purl.obolibrary.org/obo/ENVO_00000074"/>
        <obo:IAO_0000115>A barrage. Located 25 km S of Khartoum.</obo:IAO_0000115>
        <oboInOwl:hasOBONamespace>GAZ</oboInOwl:hasOBONamespace>
        <oboInOwl:id>GAZ:00256486</oboInOwl:id>
        <rdfs:label>Gebel Auliya</rdfs:label>
    </owl:NamedIndividual>
    


    <!-- http://purl.obolibrary.org/obo/GAZ_00260292 -->

    <owl:NamedIndividual rdf:about="http://purl.obolibrary.org/obo/GAZ_00260292">
        <rdf:type rdf:resource="http://purl.obolibrary.org/obo/ENVO_00000475"/>
        <obo:RO_0001025 rdf:resource="http://purl.obolibrary.org/obo/GAZ_00058791"/>
        <obo:IAO_0000115>An arm of Lake Kyoga.</obo:IAO_0000115>
        <oboInOwl:hasOBONamespace>GAZ</oboInOwl:hasOBONamespace>
        <oboInOwl:id>GAZ:00260292</oboInOwl:id>
        <rdfs:label>Mpologoma Arm</rdfs:label>
    </owl:NamedIndividual>
    


    <!-- http://purl.obolibrary.org/obo/GAZ_00281380 -->

    <owl:NamedIndividual rdf:about="http://purl.obolibrary.org/obo/GAZ_00281380">
        <obo:IAO_0000115>An island.</obo:IAO_0000115>
        <oboInOwl:hasOBONamespace>GAZ</oboInOwl:hasOBONamespace>
        <oboInOwl:id>GAZ:00281380</oboInOwl:id>
        <rdfs:label>Us Island</rdfs:label>
    </owl:NamedIndividual>
    


    <!-- http://purl.obolibrary.org/obo/GAZ_00281381 -->

    <owl:NamedIndividual rdf:about="http://purl.obolibrary.org/obo/GAZ_00281381">
        <obo:IAO_0000115>An island.</obo:IAO_0000115>
        <oboInOwl:hasOBONamespace>GAZ</oboInOwl:hasOBONamespace>
        <oboInOwl:id>GAZ:00281381</oboInOwl:id>
        <rdfs:label>Sur Island</rdfs:label>
    </owl:NamedIndividual>
    


    <!-- http://purl.obolibrary.org/obo/GAZ_00281382 -->

    <owl:NamedIndividual rdf:about="http://purl.obolibrary.org/obo/GAZ_00281382">
        <obo:IAO_0000115>An island.</obo:IAO_0000115>
        <oboInOwl:hasOBONamespace>GAZ</oboInOwl:hasOBONamespace>
        <oboInOwl:id>GAZ:00281382</oboInOwl:id>
        <rdfs:label>Sherari Island</rdfs:label>
    </owl:NamedIndividual>
    


    <!-- http://purl.obolibrary.org/obo/GAZ_00281422 -->

    <owl:NamedIndividual rdf:about="http://purl.obolibrary.org/obo/GAZ_00281422">
        <obo:IAO_0000115>A region in Libya known for extensive prehistoric rock art.</obo:IAO_0000115>
        <oboInOwl:hasOBONamespace>GAZ</oboInOwl:hasOBONamespace>
        <oboInOwl:id>GAZ:00281422</oboInOwl:id>
        <rdfs:label>Mesak Settafet</rdfs:label>
    </owl:NamedIndividual>
    


    <!-- http://purl.obolibrary.org/obo/GAZ_00281423 -->

    <owl:NamedIndividual rdf:about="http://purl.obolibrary.org/obo/GAZ_00281423">
        <obo:RO_0001025 rdf:resource="http://purl.obolibrary.org/obo/GAZ_00281422"/>
        <obo:IAO_0000115>A prehistoric archeological site in south western Libya in Mesak Settafet, famous for its rock engravings of different kinds.</obo:IAO_0000115>
        <oboInOwl:hasOBONamespace>GAZ</oboInOwl:hasOBONamespace>
        <oboInOwl:id>GAZ:00281423</oboInOwl:id>
        <rdfs:label>Wadi Mathendous</rdfs:label>
    </owl:NamedIndividual>
    


    <!-- http://purl.obolibrary.org/obo/GAZ_00281424 -->

    <owl:NamedIndividual rdf:about="http://purl.obolibrary.org/obo/GAZ_00281424">
        <obo:RO_0001025 rdf:resource="http://purl.obolibrary.org/obo/GAZ_00281422"/>
        <obo:IAO_0000115>A site of rock art.</obo:IAO_0000115>
        <oboInOwl:hasOBONamespace>GAZ</oboInOwl:hasOBONamespace>
        <oboInOwl:id>GAZ:00281424</oboInOwl:id>
        <rdfs:label>Ghalgiwan</rdfs:label>
    </owl:NamedIndividual>
    


    <!-- http://purl.obolibrary.org/obo/GAZ_00281425 -->

    <owl:NamedIndividual rdf:about="http://purl.obolibrary.org/obo/GAZ_00281425">
        <obo:RO_0001025 rdf:resource="http://purl.obolibrary.org/obo/GAZ_00281422"/>
        <obo:IAO_0000115>A site of rock art.</obo:IAO_0000115>
        <oboInOwl:hasOBONamespace>GAZ</oboInOwl:hasOBONamespace>
        <oboInOwl:id>GAZ:00281425</oboInOwl:id>
        <rdfs:label>Tiksaten</rdfs:label>
    </owl:NamedIndividual>
    


    <!-- http://purl.obolibrary.org/obo/GAZ_00281426 -->

    <owl:NamedIndividual rdf:about="http://purl.obolibrary.org/obo/GAZ_00281426">
        <obo:RO_0001025 rdf:resource="http://purl.obolibrary.org/obo/GAZ_00281422"/>
        <obo:IAO_0000115>A site of rock art.</obo:IAO_0000115>
        <oboInOwl:hasOBONamespace>GAZ</oboInOwl:hasOBONamespace>
        <oboInOwl:id>GAZ:00281426</oboInOwl:id>
        <rdfs:label>Abategh</rdfs:label>
    </owl:NamedIndividual>
    


    <!-- http://purl.obolibrary.org/obo/GAZ_00281440 -->

    <owl:NamedIndividual rdf:about="http://purl.obolibrary.org/obo/GAZ_00281440">
        <obo:RO_0001025 rdf:resource="http://purl.obolibrary.org/obo/GAZ_00000822"/>
        <obo:IAO_0000115>An archeological site. The site of the Sahara Desert&apos;s oldest known graveyard, and is located in Niger.</obo:IAO_0000115>
        <oboInOwl:hasOBONamespace>GAZ</oboInOwl:hasOBONamespace>
        <oboInOwl:id>GAZ:00281440</oboInOwl:id>
        <rdfs:label>Gobero</rdfs:label>
    </owl:NamedIndividual>
    


    <!-- http://purl.obolibrary.org/obo/GAZ_00281441 -->

    <owl:NamedIndividual rdf:about="http://purl.obolibrary.org/obo/GAZ_00281441">
        <obo:RO_0001025 rdf:resource="http://purl.obolibrary.org/obo/GAZ_00032143"/>
        <obo:IAO_0000115>An archeological site. It consists of many individual necropoleis with coffins crested by unusually-distinctive terra cotta statuettes. The main necropolis itself has a diameter of about one kilometer. Burial mounds, religious altars, and ancient dwellings occur here over a large area.</obo:IAO_0000115>
        <oboInOwl:hasOBONamespace>GAZ</oboInOwl:hasOBONamespace>
        <oboInOwl:id>GAZ:00281441</oboInOwl:id>
        <rdfs:label>Bura Archaeological Site</rdfs:label>
    </owl:NamedIndividual>
    


    <!-- 
    ///////////////////////////////////////////////////////////////////////////////////////
    //
    // Annotations
    //
    ///////////////////////////////////////////////////////////////////////////////////////
     -->

    <rdf:Description rdf:about="http://purl.obolibrary.org/obo/GAZ_00000821">
        <rdfs:label>Region (Niger)</rdfs:label>
        <oboInOwl:hasOBONamespace>GAZ</oboInOwl:hasOBONamespace>
        <oboInOwl:id>GAZ:00000821</oboInOwl:id>
    </rdf:Description>
    <rdf:Description rdf:about="http://purl.obolibrary.org/obo/GAZ_00000822">
        <obo:IAO_0000115>An administrative Region in Niger.</obo:IAO_0000115>
        <rdfs:label>Agadez Region</rdfs:label>
        <oboInOwl:hasOBONamespace>GAZ</oboInOwl:hasOBONamespace>
        <oboInOwl:id>GAZ:00000822</oboInOwl:id>
    </rdf:Description>
    <rdf:Description rdf:about="http://purl.obolibrary.org/obo/GAZ_00000823">
        <oboInOwl:hasOBONamespace>GAZ</oboInOwl:hasOBONamespace>
        <obo:IAO_0000115>An administrative Region of Niger, the capital of the region is the city of Diffa.</obo:IAO_0000115>
        <rdfs:label>Diffa Region</rdfs:label>
        <oboInOwl:id>GAZ:00000823</oboInOwl:id>
    </rdf:Description>
    <rdf:Description rdf:about="http://purl.obolibrary.org/obo/GAZ_00000824">
        <oboInOwl:hasOBONamespace>GAZ</oboInOwl:hasOBONamespace>
        <oboInOwl:id>GAZ:00000824</oboInOwl:id>
        <obo:IAO_0000115>An administrative Region of the Republic of Niger.</obo:IAO_0000115>
        <rdfs:label>Dosso Region</rdfs:label>
    </rdf:Description>
    <rdf:Description rdf:about="http://purl.obolibrary.org/obo/GAZ_00000825">
        <oboInOwl:hasOBONamespace>GAZ</oboInOwl:hasOBONamespace>
        <obo:IAO_0000115>One of eight Regions of Niger. It is located east of the Region of Tahoua and west of Zinder, in the center of Niger, north of Nigeria&apos;s city of Kano. The administrative center is at Maradi.</obo:IAO_0000115>
        <oboInOwl:id>GAZ:00000825</oboInOwl:id>
        <rdfs:label>Maradi Region</rdfs:label>
    </rdf:Description>
    <rdf:Description rdf:about="http://purl.obolibrary.org/obo/GAZ_00000826">
        <oboInOwl:hasOBONamespace>GAZ</oboInOwl:hasOBONamespace>
        <oboInOwl:id>GAZ:00000826</oboInOwl:id>
        <rdfs:label>Tahoua Region</rdfs:label>
        <obo:IAO_0000115>One of eight administrative Regions in Niger. The capital of the Region is the Commune of Tahoua.</obo:IAO_0000115>
    </rdf:Description>
    <rdf:Description rdf:about="http://purl.obolibrary.org/obo/GAZ_00000827">
        <oboInOwl:id>GAZ:00000827</oboInOwl:id>
        <oboInOwl:hasOBONamespace>GAZ</oboInOwl:hasOBONamespace>
        <obo:IAO_0000115>An administrative Region in Niger; the capital of the Region is Tillaberi.</obo:IAO_0000115>
        <rdfs:label>Tillaberi Region</rdfs:label>
    </rdf:Description>
    <rdf:Description rdf:about="http://purl.obolibrary.org/obo/GAZ_00000828">
        <rdfs:label>Zinder Region</rdfs:label>
        <oboInOwl:id>GAZ:00000828</oboInOwl:id>
        <oboInOwl:hasOBONamespace>GAZ</oboInOwl:hasOBONamespace>
        <obo:IAO_0000115>An administrative Region in Niger, the capital of the Region is the Commune of Zinder.</obo:IAO_0000115>
    </rdf:Description>
    <rdf:Description rdf:about="http://purl.obolibrary.org/obo/GAZ_00000829">
        <oboInOwl:id>GAZ:00000829</oboInOwl:id>
        <obo:IAO_0000115>The capital of Niger. It is Niger&apos;s largest city, lying on the Niger River, mostly on the east bank.</obo:IAO_0000115>
        <oboInOwl:hasOBONamespace>GAZ</oboInOwl:hasOBONamespace>
        <rdfs:label>Niamey</rdfs:label>
    </rdf:Description>
    <rdf:Description rdf:about="http://purl.obolibrary.org/obo/GAZ_00001015">
        <oboInOwl:id>GAZ:00001015</oboInOwl:id>
        <rdfs:label>Capital District (Niger)</rdfs:label>
        <oboInOwl:hasOBONamespace>GAZ</oboInOwl:hasOBONamespace>
    </rdf:Description>
    <rdf:Description rdf:about="http://purl.obolibrary.org/obo/GAZ_00058884">
        <oboInOwl:id>GAZ:00058884</oboInOwl:id>
        <obo:IAO_0000115>Shallow stretches between Aswan and Khartoum where the water&apos;s surface is broken by numerous small boulders and stones lying on the river bed, as well as many small rocky islets. In some places, these stretches are punctuated by whitewater and are perhaps well characterized as rapids, while in others the water flow is smoother.</obo:IAO_0000115>
        <oboInOwl:hasOBONamespace>GAZ</oboInOwl:hasOBONamespace>
        <rdfs:label>Cataracts of the Nile</rdfs:label>
    </rdf:Description>
    <rdf:Description rdf:about="http://purl.obolibrary.org/obo/GAZ_00058886">
        <oboInOwl:id>GAZ:00058886</oboInOwl:id>
        <obo:IAO_0000115>A cataract on the River Nile in the Manasir Desert, Sudan. It will be flooded by the Merowe Dam from 2006.</obo:IAO_0000115>
        <rdfs:label>Fourth Cataract</rdfs:label>
        <oboInOwl:hasOBONamespace>GAZ</oboInOwl:hasOBONamespace>
    </rdf:Description>
    <rdf:Description rdf:about="http://purl.obolibrary.org/obo/GAZ_00058890">
        <rdfs:label>First Cataract</rdfs:label>
        <obo:IAO_0000115>A cataract on the River Nile near Aswan.</obo:IAO_0000115>
        <oboInOwl:hasOBONamespace>GAZ</oboInOwl:hasOBONamespace>
        <oboInOwl:id>GAZ:00058890</oboInOwl:id>
    </rdf:Description>
</rdf:RDF>



<!-- Generated by the OWL API (version 4.5.6) https://github.com/owlcs/owlapi -->

