<?xml version="1.0"?>
<rdf:RDF xmlns="http://purl.obolibrary.org/obo/gaz/subsets/countries/North_Korea.owl#"
     xml:base="http://purl.obolibrary.org/obo/gaz/subsets/countries/North_Korea.owl"
     xmlns:obo="http://purl.obolibrary.org/obo/"
     xmlns:owl="http://www.w3.org/2002/07/owl#"
     xmlns:rdf="http://www.w3.org/1999/02/22-rdf-syntax-ns#"
     xmlns:xml="http://www.w3.org/XML/1998/namespace"
     xmlns:xsd="http://www.w3.org/2001/XMLSchema#"
     xmlns:rdfs="http://www.w3.org/2000/01/rdf-schema#"
     xmlns:oboInOwl="http://www.geneontology.org/formats/oboInOwl#">
    <owl:Ontology rdf:about="http://purl.obolibrary.org/obo/gaz/subsets/countries/North_Korea.owl">
        <owl:imports rdf:resource="http://purl.obolibrary.org/obo/gaz/imports/envo_import.owl"/>
        <owl:imports rdf:resource="http://purl.obolibrary.org/obo/gaz/imports/ro_import.owl"/>
    </owl:Ontology>
    


    <!-- 
    ///////////////////////////////////////////////////////////////////////////////////////
    //
    // Annotation properties
    //
    ///////////////////////////////////////////////////////////////////////////////////////
     -->

    


    <!-- http://purl.obolibrary.org/obo/IAO_0000115 -->

    <owl:AnnotationProperty rdf:about="http://purl.obolibrary.org/obo/IAO_0000115"/>
    


    <!-- http://www.geneontology.org/formats/oboInOwl#hasOBONamespace -->

    <owl:AnnotationProperty rdf:about="http://www.geneontology.org/formats/oboInOwl#hasOBONamespace"/>
    


    <!-- http://www.geneontology.org/formats/oboInOwl#id -->

    <owl:AnnotationProperty rdf:about="http://www.geneontology.org/formats/oboInOwl#id"/>
    


    <!-- 
    ///////////////////////////////////////////////////////////////////////////////////////
    //
    // Object Properties
    //
    ///////////////////////////////////////////////////////////////////////////////////////
     -->

    


    <!-- http://purl.obolibrary.org/obo/RO_0001025 -->

    <owl:ObjectProperty rdf:about="http://purl.obolibrary.org/obo/RO_0001025"/>
    


    <!-- 
    ///////////////////////////////////////////////////////////////////////////////////////
    //
    // Classes
    //
    ///////////////////////////////////////////////////////////////////////////////////////
     -->

    


    <!-- http://purl.obolibrary.org/obo/ENVO_00000004 -->

    <owl:Class rdf:about="http://purl.obolibrary.org/obo/ENVO_00000004"/>
    


    <!-- http://purl.obolibrary.org/obo/ENVO_00000009 -->

    <owl:Class rdf:about="http://purl.obolibrary.org/obo/ENVO_00000009"/>
    


    <!-- http://purl.obolibrary.org/obo/ENVO_00000029 -->

    <owl:Class rdf:about="http://purl.obolibrary.org/obo/ENVO_00000029"/>
    


    <!-- http://purl.obolibrary.org/obo/ENVO_00000074 -->

    <owl:Class rdf:about="http://purl.obolibrary.org/obo/ENVO_00000074"/>
    


    <!-- http://purl.obolibrary.org/obo/ENVO_00000220 -->

    <owl:Class rdf:about="http://purl.obolibrary.org/obo/ENVO_00000220"/>
    


    <!-- http://purl.obolibrary.org/obo/ENVO_00000856 -->

    <owl:Class rdf:about="http://purl.obolibrary.org/obo/ENVO_00000856"/>
    


    <!-- http://purl.obolibrary.org/obo/GAZ_00009238 -->

    <owl:Class rdf:about="http://purl.obolibrary.org/obo/GAZ_00009238"/>
    


    <!-- http://purl.obolibrary.org/obo/GAZ_00010088 -->

    <owl:Class rdf:about="http://purl.obolibrary.org/obo/GAZ_00010088"/>
    


    <!-- http://purl.obolibrary.org/obo/GAZ_00010089 -->

    <owl:Class rdf:about="http://purl.obolibrary.org/obo/GAZ_00010089">
        <rdfs:subClassOf rdf:resource="http://purl.obolibrary.org/obo/GAZ_00010090"/>
    </owl:Class>
    


    <!-- http://purl.obolibrary.org/obo/GAZ_00010090 -->

    <owl:Class rdf:about="http://purl.obolibrary.org/obo/GAZ_00010090"/>
    


    <!-- http://purl.obolibrary.org/obo/GAZ_00027636 -->

    <owl:Class rdf:about="http://purl.obolibrary.org/obo/GAZ_00027636">
        <rdfs:subClassOf rdf:resource="http://purl.obolibrary.org/obo/GAZ_00010090"/>
    </owl:Class>
    


    <!-- http://purl.obolibrary.org/obo/GAZ_00027637 -->

    <owl:Class rdf:about="http://purl.obolibrary.org/obo/GAZ_00027637">
        <rdfs:subClassOf rdf:resource="http://purl.obolibrary.org/obo/GAZ_00010090"/>
    </owl:Class>
    


    <!-- http://purl.obolibrary.org/obo/GAZ_00027663 -->

    <owl:Class rdf:about="http://purl.obolibrary.org/obo/GAZ_00027663">
        <rdfs:subClassOf rdf:resource="http://purl.obolibrary.org/obo/GAZ_00010090"/>
        <obo:IAO_0000115>A special administrative region of North Korea. Established 2002 to handle South Korean tourist traffic to Kumgangsan.</obo:IAO_0000115>
        <oboInOwl:hasOBONamespace>GAZ</oboInOwl:hasOBONamespace>
        <oboInOwl:id>GAZ:00027663</oboInOwl:id>
        <rdfs:label>Kumgangsan Tourist Region</rdfs:label>
    </owl:Class>
    


    <!-- http://purl.obolibrary.org/obo/GAZ_00027773 -->

    <owl:Class rdf:about="http://purl.obolibrary.org/obo/GAZ_00027773"/>
    


    <!-- http://purl.obolibrary.org/obo/GAZ_00052996 -->

    <owl:Class rdf:about="http://purl.obolibrary.org/obo/GAZ_00052996">
        <rdfs:subClassOf rdf:resource="http://purl.obolibrary.org/obo/GAZ_00010088"/>
    </owl:Class>
    


    <!-- http://purl.obolibrary.org/obo/GAZ_00128989 -->

    <owl:Class rdf:about="http://purl.obolibrary.org/obo/GAZ_00128989">
        <rdfs:subClassOf rdf:resource="http://purl.obolibrary.org/obo/GAZ_00027773"/>
    </owl:Class>
    


    <!-- http://purl.obolibrary.org/obo/GAZ_00128990 -->

    <owl:Class rdf:about="http://purl.obolibrary.org/obo/GAZ_00128990">
        <rdfs:subClassOf rdf:resource="http://purl.obolibrary.org/obo/GAZ_00027773"/>
    </owl:Class>
    


    <!-- http://purl.obolibrary.org/obo/GAZ_00128991 -->

    <owl:Class rdf:about="http://purl.obolibrary.org/obo/GAZ_00128991">
        <rdfs:subClassOf rdf:resource="http://purl.obolibrary.org/obo/GAZ_00027773"/>
    </owl:Class>
    


    <!-- http://purl.obolibrary.org/obo/GAZ_02000755 -->

    <owl:Class rdf:about="http://purl.obolibrary.org/obo/GAZ_02000755">
        <rdfs:subClassOf rdf:resource="http://purl.obolibrary.org/obo/GAZ_00010090"/>
        <obo:IAO_0000115>A special administrative industrial region of North Korea. It was formed in 2002 from part of Kaesong Directly Governed City.</obo:IAO_0000115>
        <oboInOwl:hasOBONamespace>GAZ</oboInOwl:hasOBONamespace>
        <oboInOwl:id>GAZ:02000755</oboInOwl:id>
        <rdfs:label>Kaesong Industrial Region</rdfs:label>
    </owl:Class>
    


    <!-- http://purl.obolibrary.org/obo/GAZ_02000758 -->

    <owl:Class rdf:about="http://purl.obolibrary.org/obo/GAZ_02000758">
        <rdfs:subClassOf rdf:resource="http://purl.obolibrary.org/obo/GAZ_00009238"/>
    </owl:Class>
    


    <!-- http://purl.obolibrary.org/obo/GAZ_02000759 -->

    <owl:Class rdf:about="http://purl.obolibrary.org/obo/GAZ_02000759">
        <rdfs:subClassOf rdf:resource="http://purl.obolibrary.org/obo/GAZ_00009238"/>
    </owl:Class>
    


    <!-- http://purl.obolibrary.org/obo/GAZ_02000760 -->

    <owl:Class rdf:about="http://purl.obolibrary.org/obo/GAZ_02000760">
        <rdfs:subClassOf rdf:resource="http://purl.obolibrary.org/obo/GAZ_00009238"/>
    </owl:Class>
    


    <!-- http://purl.obolibrary.org/obo/GAZ_02000761 -->

    <owl:Class rdf:about="http://purl.obolibrary.org/obo/GAZ_02000761">
        <rdfs:subClassOf rdf:resource="http://purl.obolibrary.org/obo/GAZ_00009238"/>
    </owl:Class>
    


    <!-- http://purl.obolibrary.org/obo/GAZ_02000762 -->

    <owl:Class rdf:about="http://purl.obolibrary.org/obo/GAZ_02000762">
        <rdfs:subClassOf rdf:resource="http://purl.obolibrary.org/obo/GAZ_00009238"/>
    </owl:Class>
    


    <!-- http://purl.obolibrary.org/obo/GAZ_02000763 -->

    <owl:Class rdf:about="http://purl.obolibrary.org/obo/GAZ_02000763">
        <rdfs:subClassOf rdf:resource="http://purl.obolibrary.org/obo/GAZ_00009238"/>
    </owl:Class>
    


    <!-- http://purl.obolibrary.org/obo/GAZ_02000764 -->

    <owl:Class rdf:about="http://purl.obolibrary.org/obo/GAZ_02000764">
        <rdfs:subClassOf rdf:resource="http://purl.obolibrary.org/obo/GAZ_00009238"/>
    </owl:Class>
    


    <!-- http://purl.obolibrary.org/obo/GAZ_02000765 -->

    <owl:Class rdf:about="http://purl.obolibrary.org/obo/GAZ_02000765">
        <rdfs:subClassOf rdf:resource="http://purl.obolibrary.org/obo/GAZ_00009238"/>
    </owl:Class>
    


    <!-- http://purl.obolibrary.org/obo/GAZ_02000766 -->

    <owl:Class rdf:about="http://purl.obolibrary.org/obo/GAZ_02000766">
        <rdfs:subClassOf rdf:resource="http://purl.obolibrary.org/obo/GAZ_00009238"/>
    </owl:Class>
    


    <!-- 
    ///////////////////////////////////////////////////////////////////////////////////////
    //
    // Individuals
    //
    ///////////////////////////////////////////////////////////////////////////////////////
     -->

    


    <!-- http://purl.obolibrary.org/obo/GAZ_00002801 -->

    <owl:NamedIndividual rdf:about="http://purl.obolibrary.org/obo/GAZ_00002801">
        <rdf:type rdf:resource="http://purl.obolibrary.org/obo/ENVO_00000009"/>
        <obo:IAO_0000115>A state in East Asia in the northern half of the Korean Peninsula, with its capital in the city of Pyongyang. To the south and separated by the Korean Demilitarized Zone is South Korea, with which it formed one nation until division following World War II. At its northern Amnok River border are China and, separated by the Tumen River in the extreme north-east, Russia.</obo:IAO_0000115>
        <oboInOwl:hasOBONamespace>GAZ</oboInOwl:hasOBONamespace>
        <oboInOwl:id>GAZ:00002801</oboInOwl:id>
        <rdfs:label>North Korea</rdfs:label>
    </owl:NamedIndividual>
    


    <!-- http://purl.obolibrary.org/obo/GAZ_00009238 -->

    <owl:NamedIndividual rdf:about="http://purl.obolibrary.org/obo/GAZ_00009238">
        <obo:RO_0001025 rdf:resource="http://purl.obolibrary.org/obo/GAZ_00002801"/>
    </owl:NamedIndividual>
    


    <!-- http://purl.obolibrary.org/obo/GAZ_00010088 -->

    <owl:NamedIndividual rdf:about="http://purl.obolibrary.org/obo/GAZ_00010088">
        <obo:RO_0001025 rdf:resource="http://purl.obolibrary.org/obo/GAZ_00002801"/>
    </owl:NamedIndividual>
    


    <!-- http://purl.obolibrary.org/obo/GAZ_00010089 -->

    <owl:NamedIndividual rdf:about="http://purl.obolibrary.org/obo/GAZ_00010089"/>
    


    <!-- http://purl.obolibrary.org/obo/GAZ_00010090 -->

    <owl:NamedIndividual rdf:about="http://purl.obolibrary.org/obo/GAZ_00010090">
        <obo:RO_0001025 rdf:resource="http://purl.obolibrary.org/obo/GAZ_00002801"/>
    </owl:NamedIndividual>
    


    <!-- http://purl.obolibrary.org/obo/GAZ_00027632 -->

    <owl:NamedIndividual rdf:about="http://purl.obolibrary.org/obo/GAZ_00027632">
        <obo:RO_0001025 rdf:resource="http://purl.obolibrary.org/obo/GAZ_00010089"/>
        <obo:IAO_0000115>One of the four suburban counties of Pyongyang, North Korea. It is north-west of Songrim-si, North Hwanghae Province, north-east of Hwangju-gun, North Hwangae Province, west of Chunghwa-gun, Pyongyang and south of Rakrang-guyok, Pyongyang. It became part of Pyongyang in 1963-05, when it was separated from P&apos;yongan-nam Province.</obo:IAO_0000115>
        <oboInOwl:hasOBONamespace>GAZ</oboInOwl:hasOBONamespace>
        <oboInOwl:id>GAZ:00027632</oboInOwl:id>
        <rdfs:label>Kangnam County</rdfs:label>
    </owl:NamedIndividual>
    


    <!-- http://purl.obolibrary.org/obo/GAZ_00027633 -->

    <owl:NamedIndividual rdf:about="http://purl.obolibrary.org/obo/GAZ_00027633">
        <obo:RO_0001025 rdf:resource="http://purl.obolibrary.org/obo/GAZ_00010089"/>
        <obo:IAO_0000115>One of the four suburban counties located in east Pyongyang, North Korea. It became part of Pyongyang in 1963-05 when it was separated from P&apos;yongan-nam Province. It is north of Hwangju-gun, Yontan-gun and Suan-gun North Hwanghae Province, south of the Nam River and Kangdong-gun, Pyongyang, west of Yonsan-gun North Hwanghae Province and east of Chunghwa-gun, Pyongyang.</obo:IAO_0000115>
        <oboInOwl:hasOBONamespace>GAZ</oboInOwl:hasOBONamespace>
        <oboInOwl:id>GAZ:00027633</oboInOwl:id>
        <rdfs:label>Sangwon County</rdfs:label>
    </owl:NamedIndividual>
    


    <!-- http://purl.obolibrary.org/obo/GAZ_00027634 -->

    <owl:NamedIndividual rdf:about="http://purl.obolibrary.org/obo/GAZ_00027634">
        <obo:RO_0001025 rdf:resource="http://purl.obolibrary.org/obo/GAZ_00010089"/>
        <obo:IAO_0000115>One of Pyongyang&apos;s four suburban counties. In 1983 it was separated from P&apos;yongan-nam Province and assumed direct governance by the Pyongyang. It is bordered by Songch&apos;on-gun (Songchon County), P&apos;yongan-nam in the north and east, Songho-guyok (Sungho District) from the south and the Taedong River from the west.</obo:IAO_0000115>
        <oboInOwl:hasOBONamespace>GAZ</oboInOwl:hasOBONamespace>
        <oboInOwl:id>GAZ:00027634</oboInOwl:id>
        <rdfs:label>Kangdong County</rdfs:label>
    </owl:NamedIndividual>
    


    <!-- http://purl.obolibrary.org/obo/GAZ_00027635 -->

    <owl:NamedIndividual rdf:about="http://purl.obolibrary.org/obo/GAZ_00027635">
        <obo:RO_0001025 rdf:resource="http://purl.obolibrary.org/obo/GAZ_00010089"/>
        <obo:IAO_0000115>One of the four suburban counties of East Pyongyang, North Korea. It sits north of Hwangju-gun, North Hwanghae Province, east of Kangnam-gun, Pyongyang, west of Sangwon-gun, Pyongyang and south of Ryokp&apos;o-guyok, Pyongyang. It became part of Pyongyang in 1963-05, when it separated from P&apos;yongan-nam Province.</obo:IAO_0000115>
        <oboInOwl:hasOBONamespace>GAZ</oboInOwl:hasOBONamespace>
        <oboInOwl:id>GAZ:00027635</oboInOwl:id>
        <rdfs:label>Chunghwa County</rdfs:label>
    </owl:NamedIndividual>
    


    <!-- http://purl.obolibrary.org/obo/GAZ_00027636 -->

    <owl:NamedIndividual rdf:about="http://purl.obolibrary.org/obo/GAZ_00027636"/>
    


    <!-- http://purl.obolibrary.org/obo/GAZ_00027637 -->

    <owl:NamedIndividual rdf:about="http://purl.obolibrary.org/obo/GAZ_00027637"/>
    


    <!-- http://purl.obolibrary.org/obo/GAZ_00027639 -->

    <owl:NamedIndividual rdf:about="http://purl.obolibrary.org/obo/GAZ_00027639">
        <obo:RO_0001025 rdf:resource="http://purl.obolibrary.org/obo/GAZ_02000759"/>
        <obo:IAO_0000115>A county in P&apos;yongan-buk Province, North Korea. Sakchu and Kusong counties lie to the east; Sonch&apos;on and Ch&apos;olsan counties to the south; and Ryongch&apos;on county and Sinuiju to the west. To the north, Uiju shares a border with China. Partly in Sinuiju Special Administrative Region.</obo:IAO_0000115>
        <oboInOwl:hasOBONamespace>GAZ</oboInOwl:hasOBONamespace>
        <oboInOwl:id>GAZ:00027639</oboInOwl:id>
        <rdfs:label>Uiju County</rdfs:label>
    </owl:NamedIndividual>
    


    <!-- http://purl.obolibrary.org/obo/GAZ_00027642 -->

    <owl:NamedIndividual rdf:about="http://purl.obolibrary.org/obo/GAZ_00027642">
        <obo:RO_0001025 rdf:resource="http://purl.obolibrary.org/obo/GAZ_00129023"/>
        <obo:IAO_0000115>One of the 19 guyok that constitute Pyongyang, North Korea.</obo:IAO_0000115>
        <oboInOwl:hasOBONamespace>GAZ</oboInOwl:hasOBONamespace>
        <oboInOwl:id>GAZ:00027642</oboInOwl:id>
        <rdfs:label>Ryokp&apos;o District</rdfs:label>
    </owl:NamedIndividual>
    


    <!-- http://purl.obolibrary.org/obo/GAZ_00027643 -->

    <owl:NamedIndividual rdf:about="http://purl.obolibrary.org/obo/GAZ_00027643">
        <obo:RO_0001025 rdf:resource="http://purl.obolibrary.org/obo/GAZ_00129023"/>
        <obo:IAO_0000115>One of the 19 guyok (political districts or wards) of Pyongyang, North Korea. It is situated on the Taedong River in the South and the Pot&apos;ong River in the north. It is east of Chung-guyok, separated by the railway. It was established as a guyok in 1960-10.</obo:IAO_0000115>
        <oboInOwl:hasOBONamespace>GAZ</oboInOwl:hasOBONamespace>
        <oboInOwl:id>GAZ:00027643</oboInOwl:id>
        <rdfs:label>Phyongchon District</rdfs:label>
    </owl:NamedIndividual>
    


    <!-- http://purl.obolibrary.org/obo/GAZ_00027644 -->

    <owl:NamedIndividual rdf:about="http://purl.obolibrary.org/obo/GAZ_00027644">
        <obo:RO_0001025 rdf:resource="http://purl.obolibrary.org/obo/GAZ_00129023"/>
        <obo:IAO_0000115>One of the 19 guyok that constitute Pyongyang, North Korea.</obo:IAO_0000115>
        <oboInOwl:hasOBONamespace>GAZ</oboInOwl:hasOBONamespace>
        <oboInOwl:id>GAZ:00027644</oboInOwl:id>
        <rdfs:label>Unjong District</rdfs:label>
    </owl:NamedIndividual>
    


    <!-- http://purl.obolibrary.org/obo/GAZ_00027645 -->

    <owl:NamedIndividual rdf:about="http://purl.obolibrary.org/obo/GAZ_00027645">
        <obo:RO_0001025 rdf:resource="http://purl.obolibrary.org/obo/GAZ_00129023"/>
        <obo:IAO_0000115>One of the 19 guyok that constitute Pyongyang, North Korea. It is located north of Chung-guyok or the Central District and south of Taesong-guyok, Taesong District. It was designated a guyok in 1960-10.</obo:IAO_0000115>
        <oboInOwl:hasOBONamespace>GAZ</oboInOwl:hasOBONamespace>
        <oboInOwl:id>GAZ:00027645</oboInOwl:id>
        <rdfs:label>Moranbong District</rdfs:label>
    </owl:NamedIndividual>
    


    <!-- http://purl.obolibrary.org/obo/GAZ_00027646 -->

    <owl:NamedIndividual rdf:about="http://purl.obolibrary.org/obo/GAZ_00027646">
        <obo:RO_0001025 rdf:resource="http://purl.obolibrary.org/obo/GAZ_00129023"/>
        <obo:IAO_0000115>One of the 19 guyok that constitute Pyongyang, North Korea.</obo:IAO_0000115>
        <oboInOwl:hasOBONamespace>GAZ</oboInOwl:hasOBONamespace>
        <oboInOwl:id>GAZ:00027646</oboInOwl:id>
        <rdfs:label>Ryongsong District</rdfs:label>
    </owl:NamedIndividual>
    


    <!-- http://purl.obolibrary.org/obo/GAZ_00027647 -->

    <owl:NamedIndividual rdf:about="http://purl.obolibrary.org/obo/GAZ_00027647">
        <obo:RO_0001025 rdf:resource="http://purl.obolibrary.org/obo/GAZ_00129023"/>
        <obo:IAO_0000115>One of the 19 guyok, and one of the six, that constitute East Pyongyang, North Korea. It is on the eastern bank of the Taedong River, and the mouth of the Nam River. It is north of Ryokp&apos;o-guyok (Ryokpho District), east of Taedonggang-guyok (Taedonggang District) and north east of Tongdaewon-guyok. Established 1959-09.</obo:IAO_0000115>
        <oboInOwl:hasOBONamespace>GAZ</oboInOwl:hasOBONamespace>
        <oboInOwl:id>GAZ:00027647</oboInOwl:id>
        <rdfs:label>Sadong District</rdfs:label>
    </owl:NamedIndividual>
    


    <!-- http://purl.obolibrary.org/obo/GAZ_00027648 -->

    <owl:NamedIndividual rdf:about="http://purl.obolibrary.org/obo/GAZ_00027648">
        <obo:RO_0001025 rdf:resource="http://purl.obolibrary.org/obo/GAZ_00129023"/>
        <obo:IAO_0000115>The Central District of Pyongyang, the capital of North Korea.</obo:IAO_0000115>
        <oboInOwl:hasOBONamespace>GAZ</oboInOwl:hasOBONamespace>
        <oboInOwl:id>GAZ:00027648</oboInOwl:id>
        <rdfs:label>Chung District</rdfs:label>
    </owl:NamedIndividual>
    


    <!-- http://purl.obolibrary.org/obo/GAZ_00027649 -->

    <owl:NamedIndividual rdf:about="http://purl.obolibrary.org/obo/GAZ_00027649">
        <obo:RO_0001025 rdf:resource="http://purl.obolibrary.org/obo/GAZ_00129023"/>
        <obo:IAO_0000115>One of the 19 guyok of Pyongyang, North Korea. It is located on the Pot&apos;ong River, west of the Moranbong-guyok (Moranbong District) and south of Hyongjesan-guyok (Hyongjesan District). It was established 1958-01.</obo:IAO_0000115>
        <oboInOwl:hasOBONamespace>GAZ</oboInOwl:hasOBONamespace>
        <oboInOwl:id>GAZ:00027649</oboInOwl:id>
        <rdfs:label>Sosong District</rdfs:label>
    </owl:NamedIndividual>
    


    <!-- http://purl.obolibrary.org/obo/GAZ_00027650 -->

    <owl:NamedIndividual rdf:about="http://purl.obolibrary.org/obo/GAZ_00027650">
        <obo:RO_0001025 rdf:resource="http://purl.obolibrary.org/obo/GAZ_00129023"/>
        <obo:IAO_0000115>One of the 19 guyok of Pyongyang, North Korea.</obo:IAO_0000115>
        <oboInOwl:hasOBONamespace>GAZ</oboInOwl:hasOBONamespace>
        <oboInOwl:id>GAZ:00027650</oboInOwl:id>
        <rdfs:label>Pot&apos;onggang District</rdfs:label>
    </owl:NamedIndividual>
    


    <!-- http://purl.obolibrary.org/obo/GAZ_00027651 -->

    <owl:NamedIndividual rdf:about="http://purl.obolibrary.org/obo/GAZ_00027651">
        <obo:RO_0001025 rdf:resource="http://purl.obolibrary.org/obo/GAZ_00129023"/>
        <obo:IAO_0000115>One of the 19 guyok that constitute Pyongyang, North Korea.</obo:IAO_0000115>
        <oboInOwl:hasOBONamespace>GAZ</oboInOwl:hasOBONamespace>
        <oboInOwl:id>GAZ:00027651</oboInOwl:id>
        <rdfs:label>Samsok District</rdfs:label>
    </owl:NamedIndividual>
    


    <!-- http://purl.obolibrary.org/obo/GAZ_00027652 -->

    <owl:NamedIndividual rdf:about="http://purl.obolibrary.org/obo/GAZ_00027652">
        <obo:RO_0001025 rdf:resource="http://purl.obolibrary.org/obo/GAZ_00129023"/>
        <obo:IAO_0000115>One of the 19 guyok that constitute Pyongyang, North Korea.</obo:IAO_0000115>
        <oboInOwl:hasOBONamespace>GAZ</oboInOwl:hasOBONamespace>
        <oboInOwl:id>GAZ:00027652</oboInOwl:id>
        <rdfs:label>Sunan District</rdfs:label>
    </owl:NamedIndividual>
    


    <!-- http://purl.obolibrary.org/obo/GAZ_00027653 -->

    <owl:NamedIndividual rdf:about="http://purl.obolibrary.org/obo/GAZ_00027653">
        <obo:RO_0001025 rdf:resource="http://purl.obolibrary.org/obo/GAZ_00129023"/>
        <obo:IAO_0000115>One of the 19 guyok, and one of the six that constitute East Pyongyang, North Korea. It sits on the eastern bank of the Taedong River. It is north of Son&apos;gyo-guyok (Songyo District), south of Taedonggang-guyok (Taedonggang District) and west of Sadong-guyok (Sadong District) and Ryokp&apos;o-guyok (Ryokpho District). Established 1960-10.</obo:IAO_0000115>
        <oboInOwl:hasOBONamespace>GAZ</oboInOwl:hasOBONamespace>
        <oboInOwl:id>GAZ:00027653</oboInOwl:id>
        <rdfs:label>Tongdaewon District</rdfs:label>
    </owl:NamedIndividual>
    


    <!-- http://purl.obolibrary.org/obo/GAZ_00027654 -->

    <owl:NamedIndividual rdf:about="http://purl.obolibrary.org/obo/GAZ_00027654">
        <obo:RO_0001025 rdf:resource="http://purl.obolibrary.org/obo/GAZ_00129023"/>
        <obo:IAO_0000115>One of the 19 guyok that constitute Pyongyang, North Korea.</obo:IAO_0000115>
        <oboInOwl:hasOBONamespace>GAZ</oboInOwl:hasOBONamespace>
        <oboInOwl:id>GAZ:00027654</oboInOwl:id>
        <rdfs:label>Sungho District</rdfs:label>
    </owl:NamedIndividual>
    


    <!-- http://purl.obolibrary.org/obo/GAZ_00027655 -->

    <owl:NamedIndividual rdf:about="http://purl.obolibrary.org/obo/GAZ_00027655">
        <obo:RO_0001025 rdf:resource="http://purl.obolibrary.org/obo/GAZ_00129023"/>
        <obo:IAO_0000115>One of the 19 guyok, and one of the six that constitute East Pyongyang, North Korea. Taedonggang-guyok is on the eastern bank of the Taedong River, north of Tongdaewon-guyok and west of Sadong-guyok (Sadong District). Established 1958-01.</obo:IAO_0000115>
        <oboInOwl:hasOBONamespace>GAZ</oboInOwl:hasOBONamespace>
        <oboInOwl:id>GAZ:00027655</oboInOwl:id>
        <rdfs:label>Taedonggang District</rdfs:label>
    </owl:NamedIndividual>
    


    <!-- http://purl.obolibrary.org/obo/GAZ_00027656 -->

    <owl:NamedIndividual rdf:about="http://purl.obolibrary.org/obo/GAZ_00027656">
        <obo:RO_0001025 rdf:resource="http://purl.obolibrary.org/obo/GAZ_00129023"/>
        <obo:IAO_0000115>One of the 19 guyok that constitute Pyongyang, North Korea.</obo:IAO_0000115>
        <oboInOwl:hasOBONamespace>GAZ</oboInOwl:hasOBONamespace>
        <oboInOwl:id>GAZ:00027656</oboInOwl:id>
        <rdfs:label>Taesong District</rdfs:label>
    </owl:NamedIndividual>
    


    <!-- http://purl.obolibrary.org/obo/GAZ_00027657 -->

    <owl:NamedIndividual rdf:about="http://purl.obolibrary.org/obo/GAZ_00027657">
        <obo:RO_0001025 rdf:resource="http://purl.obolibrary.org/obo/GAZ_00129023"/>
        <obo:IAO_0000115>One of the 19 guyok that constitute Pyongyang, North Korea.</obo:IAO_0000115>
        <oboInOwl:hasOBONamespace>GAZ</oboInOwl:hasOBONamespace>
        <oboInOwl:id>GAZ:00027657</oboInOwl:id>
        <rdfs:label>Man&apos;gyongdae District</rdfs:label>
    </owl:NamedIndividual>
    


    <!-- http://purl.obolibrary.org/obo/GAZ_00027658 -->

    <owl:NamedIndividual rdf:about="http://purl.obolibrary.org/obo/GAZ_00027658">
        <obo:RO_0001025 rdf:resource="http://purl.obolibrary.org/obo/GAZ_00129023"/>
        <obo:IAO_0000115>Ane of the 19 guyok of Pyongyang, North Korea. It is on the eastern bank of the Taedong River and is of the six districts and four counties that constitute East Pyongyang. It is north east of Rangrang-guyok, south of Tongdaewon-guyok (Tongdaewon District) and west of Ryokp&apos;o-guyok (Ryokp&apos;o District) Sadong-guyok (Sadong District). Established 1959-09.</obo:IAO_0000115>
        <oboInOwl:hasOBONamespace>GAZ</oboInOwl:hasOBONamespace>
        <oboInOwl:id>GAZ:00027658</oboInOwl:id>
        <rdfs:label>Son&apos;gyo District</rdfs:label>
    </owl:NamedIndividual>
    


    <!-- http://purl.obolibrary.org/obo/GAZ_00027659 -->

    <owl:NamedIndividual rdf:about="http://purl.obolibrary.org/obo/GAZ_00027659">
        <obo:RO_0001025 rdf:resource="http://purl.obolibrary.org/obo/GAZ_00129023"/>
        <obo:IAO_0000115>One of the 19 guyok that constitute Pyongyang, North Korea.</obo:IAO_0000115>
        <oboInOwl:hasOBONamespace>GAZ</oboInOwl:hasOBONamespace>
        <oboInOwl:id>GAZ:00027659</oboInOwl:id>
        <rdfs:label>Rakrang District</rdfs:label>
    </owl:NamedIndividual>
    


    <!-- http://purl.obolibrary.org/obo/GAZ_00027660 -->

    <owl:NamedIndividual rdf:about="http://purl.obolibrary.org/obo/GAZ_00027660">
        <obo:RO_0001025 rdf:resource="http://purl.obolibrary.org/obo/GAZ_00129023"/>
        <obo:IAO_0000115>One of the 19 guyok that constitute Pyongyang, North Korea.</obo:IAO_0000115>
        <oboInOwl:hasOBONamespace>GAZ</oboInOwl:hasOBONamespace>
        <oboInOwl:id>GAZ:00027660</oboInOwl:id>
        <rdfs:label>Hyongjesan District</rdfs:label>
    </owl:NamedIndividual>
    


    <!-- http://purl.obolibrary.org/obo/GAZ_00027661 -->

    <owl:NamedIndividual rdf:about="http://purl.obolibrary.org/obo/GAZ_00027661">
        <rdf:type rdf:resource="http://purl.obolibrary.org/obo/ENVO_00000004"/>
        <obo:RO_0001025 rdf:resource="http://purl.obolibrary.org/obo/GAZ_00027636"/>
        <obo:IAO_0000115>A district of Rajin.</obo:IAO_0000115>
        <oboInOwl:hasOBONamespace>GAZ</oboInOwl:hasOBONamespace>
        <oboInOwl:id>GAZ:00027661</oboInOwl:id>
        <rdfs:label>Rajin District</rdfs:label>
    </owl:NamedIndividual>
    


    <!-- http://purl.obolibrary.org/obo/GAZ_00027662 -->

    <owl:NamedIndividual rdf:about="http://purl.obolibrary.org/obo/GAZ_00027662">
        <obo:RO_0001025 rdf:resource="http://purl.obolibrary.org/obo/GAZ_00027636"/>
        <obo:IAO_0000115>A subdivision of the North Korean city of Rason. It is located at the northeastern extreme of North Korea, bordering Russia and China. It lies on Unggi Bay, an extension of the Sea of Japan (East Sea of Korea).</obo:IAO_0000115>
        <oboInOwl:hasOBONamespace>GAZ</oboInOwl:hasOBONamespace>
        <oboInOwl:id>GAZ:00027662</oboInOwl:id>
        <rdfs:label>Sonbong County</rdfs:label>
    </owl:NamedIndividual>
    


    <!-- http://purl.obolibrary.org/obo/GAZ_00027664 -->

    <owl:NamedIndividual rdf:about="http://purl.obolibrary.org/obo/GAZ_00027664">
        <obo:RO_0001025 rdf:resource="http://purl.obolibrary.org/obo/GAZ_02000765"/>
        <obo:IAO_0000115>A county of P&apos;yongan-nam Province. It is bordered to the north by Yongrim and Changjin, to the east by Yonggwang and Hamju, to the south by Yodok and Chongpyong, and to the west by Yongwon and Tongsin. It is drained by the Taedong River.</obo:IAO_0000115>
        <oboInOwl:hasOBONamespace>GAZ</oboInOwl:hasOBONamespace>
        <oboInOwl:id>GAZ:00027664</oboInOwl:id>
        <rdfs:label>Taehung County</rdfs:label>
    </owl:NamedIndividual>
    


    <!-- http://purl.obolibrary.org/obo/GAZ_00027665 -->

    <owl:NamedIndividual rdf:about="http://purl.obolibrary.org/obo/GAZ_00027665">
        <obo:RO_0001025 rdf:resource="http://purl.obolibrary.org/obo/GAZ_02000765"/>
        <obo:IAO_0000115>A populated place. A city in North Korea, the capital city of P&apos;yongan-nam Province in western North Korea.</obo:IAO_0000115>
        <oboInOwl:hasOBONamespace>GAZ</oboInOwl:hasOBONamespace>
        <oboInOwl:id>GAZ:00027665</oboInOwl:id>
        <rdfs:label>P&apos;yongsong City</rdfs:label>
    </owl:NamedIndividual>
    


    <!-- http://purl.obolibrary.org/obo/GAZ_00027666 -->

    <owl:NamedIndividual rdf:about="http://purl.obolibrary.org/obo/GAZ_00027666">
        <rdf:type rdf:resource="http://purl.obolibrary.org/obo/ENVO_00000004"/>
        <obo:RO_0001025 rdf:resource="http://purl.obolibrary.org/obo/GAZ_02000765"/>
        <obo:IAO_0000115>A district of P&apos;yongan-nam Province.</obo:IAO_0000115>
        <oboInOwl:hasOBONamespace>GAZ</oboInOwl:hasOBONamespace>
        <oboInOwl:id>GAZ:00027666</oboInOwl:id>
        <rdfs:label>Tukchang District</rdfs:label>
    </owl:NamedIndividual>
    


    <!-- http://purl.obolibrary.org/obo/GAZ_00027667 -->

    <owl:NamedIndividual rdf:about="http://purl.obolibrary.org/obo/GAZ_00027667">
        <obo:RO_0001025 rdf:resource="http://purl.obolibrary.org/obo/GAZ_02000765"/>
        <obo:IAO_0000115>A city of P&apos;yongan-nam Province in western North Korea.</obo:IAO_0000115>
        <oboInOwl:hasOBONamespace>GAZ</oboInOwl:hasOBONamespace>
        <oboInOwl:id>GAZ:00027667</oboInOwl:id>
        <rdfs:label>Sunch&apos;on City</rdfs:label>
    </owl:NamedIndividual>
    


    <!-- http://purl.obolibrary.org/obo/GAZ_00027668 -->

    <owl:NamedIndividual rdf:about="http://purl.obolibrary.org/obo/GAZ_00027668">
        <rdf:type rdf:resource="http://purl.obolibrary.org/obo/ENVO_00000004"/>
        <obo:RO_0001025 rdf:resource="http://purl.obolibrary.org/obo/GAZ_02000765"/>
        <obo:IAO_0000115>A district of P&apos;yongan-nam Province.</obo:IAO_0000115>
        <oboInOwl:hasOBONamespace>GAZ</oboInOwl:hasOBONamespace>
        <oboInOwl:id>GAZ:00027668</oboInOwl:id>
        <rdfs:label>Ch&apos;ongnam District</rdfs:label>
    </owl:NamedIndividual>
    


    <!-- http://purl.obolibrary.org/obo/GAZ_00027669 -->

    <owl:NamedIndividual rdf:about="http://purl.obolibrary.org/obo/GAZ_00027669">
        <obo:RO_0001025 rdf:resource="http://purl.obolibrary.org/obo/GAZ_02000765"/>
        <obo:IAO_0000115>A city of P&apos;yongan-nam Province in western North Korea. The Ch&apos;ongch&apos;on River passes through Anju.</obo:IAO_0000115>
        <oboInOwl:hasOBONamespace>GAZ</oboInOwl:hasOBONamespace>
        <oboInOwl:id>GAZ:00027669</oboInOwl:id>
        <rdfs:label>Anju City</rdfs:label>
    </owl:NamedIndividual>
    


    <!-- http://purl.obolibrary.org/obo/GAZ_00027670 -->

    <owl:NamedIndividual rdf:about="http://purl.obolibrary.org/obo/GAZ_00027670">
        <obo:RO_0001025 rdf:resource="http://purl.obolibrary.org/obo/GAZ_02000765"/>
        <obo:IAO_0000115>A county of P&apos;yongan-nam Province.</obo:IAO_0000115>
        <oboInOwl:hasOBONamespace>GAZ</oboInOwl:hasOBONamespace>
        <oboInOwl:id>GAZ:00027670</oboInOwl:id>
        <rdfs:label>Yangdok County</rdfs:label>
    </owl:NamedIndividual>
    


    <!-- http://purl.obolibrary.org/obo/GAZ_00027671 -->

    <owl:NamedIndividual rdf:about="http://purl.obolibrary.org/obo/GAZ_00027671">
        <obo:RO_0001025 rdf:resource="http://purl.obolibrary.org/obo/GAZ_02000765"/>
        <obo:IAO_0000115>A city of P&apos;yongan-nam Province in western North Korea. It is bordered by Yongwon and Maengsan to the east, Kujang to the north, Kaechon to the west and Pukchang to the south.</obo:IAO_0000115>
        <oboInOwl:hasOBONamespace>GAZ</oboInOwl:hasOBONamespace>
        <oboInOwl:id>GAZ:00027671</oboInOwl:id>
        <rdfs:label>Tokch&apos;on City</rdfs:label>
    </owl:NamedIndividual>
    


    <!-- http://purl.obolibrary.org/obo/GAZ_00027672 -->

    <owl:NamedIndividual rdf:about="http://purl.obolibrary.org/obo/GAZ_00027672">
        <rdf:type rdf:resource="http://purl.obolibrary.org/obo/ENVO_00000004"/>
        <obo:RO_0001025 rdf:resource="http://purl.obolibrary.org/obo/GAZ_02000765"/>
        <obo:IAO_0000115>A district of P&apos;yongan-nam Province.</obo:IAO_0000115>
        <oboInOwl:hasOBONamespace>GAZ</oboInOwl:hasOBONamespace>
        <oboInOwl:id>GAZ:00027672</oboInOwl:id>
        <rdfs:label>Ungok District</rdfs:label>
    </owl:NamedIndividual>
    


    <!-- http://purl.obolibrary.org/obo/GAZ_00027673 -->

    <owl:NamedIndividual rdf:about="http://purl.obolibrary.org/obo/GAZ_00027673">
        <obo:RO_0001025 rdf:resource="http://purl.obolibrary.org/obo/GAZ_02000765"/>
        <obo:IAO_0000115>A city of P&apos;yongan-nam Province in western North Korea.</obo:IAO_0000115>
        <oboInOwl:hasOBONamespace>GAZ</oboInOwl:hasOBONamespace>
        <oboInOwl:id>GAZ:00027673</oboInOwl:id>
        <rdfs:label>Kaech&apos;on City</rdfs:label>
    </owl:NamedIndividual>
    


    <!-- http://purl.obolibrary.org/obo/GAZ_00027674 -->

    <owl:NamedIndividual rdf:about="http://purl.obolibrary.org/obo/GAZ_00027674">
        <obo:RO_0001025 rdf:resource="http://purl.obolibrary.org/obo/GAZ_02000765"/>
        <obo:IAO_0000115>A county of P&apos;yongan-nam Province. It borders Hyangsan in the east, Kujang and Nyongbyon in the south, and Tongchang and Taechon in the west. In addition, it is bordered by Chagang province to the east (Huichon) and north (Songwon).</obo:IAO_0000115>
        <oboInOwl:hasOBONamespace>GAZ</oboInOwl:hasOBONamespace>
        <oboInOwl:id>GAZ:00027674</oboInOwl:id>
        <rdfs:label>Unsan County</rdfs:label>
    </owl:NamedIndividual>
    


    <!-- http://purl.obolibrary.org/obo/GAZ_00027675 -->

    <owl:NamedIndividual rdf:about="http://purl.obolibrary.org/obo/GAZ_00027675">
        <obo:RO_0001025 rdf:resource="http://purl.obolibrary.org/obo/GAZ_02000765"/>
        <obo:IAO_0000115>A county of P&apos;yongan-nam Province.</obo:IAO_0000115>
        <oboInOwl:hasOBONamespace>GAZ</oboInOwl:hasOBONamespace>
        <oboInOwl:id>GAZ:00027675</oboInOwl:id>
        <rdfs:label>Pukch&apos;ang County</rdfs:label>
    </owl:NamedIndividual>
    


    <!-- http://purl.obolibrary.org/obo/GAZ_00027676 -->

    <owl:NamedIndividual rdf:about="http://purl.obolibrary.org/obo/GAZ_00027676">
        <obo:RO_0001025 rdf:resource="http://purl.obolibrary.org/obo/GAZ_02000765"/>
        <obo:IAO_0000115>A county of P&apos;yongan-nam Province.</obo:IAO_0000115>
        <oboInOwl:hasOBONamespace>GAZ</oboInOwl:hasOBONamespace>
        <oboInOwl:id>GAZ:00027676</oboInOwl:id>
        <rdfs:label>Onch&apos;on County</rdfs:label>
    </owl:NamedIndividual>
    


    <!-- http://purl.obolibrary.org/obo/GAZ_00027677 -->

    <owl:NamedIndividual rdf:about="http://purl.obolibrary.org/obo/GAZ_00027677">
        <obo:RO_0001025 rdf:resource="http://purl.obolibrary.org/obo/GAZ_00057403"/>
        <obo:RO_0001025 rdf:resource="http://purl.obolibrary.org/obo/GAZ_02000762"/>
        <obo:IAO_0000115>A county in Ryanggang province, North Korea. Kapsan lies on the eastern edge of the Kaema Plateau.</obo:IAO_0000115>
        <oboInOwl:hasOBONamespace>GAZ</oboInOwl:hasOBONamespace>
        <oboInOwl:id>GAZ:00027677</oboInOwl:id>
        <rdfs:label>Kapsan County</rdfs:label>
    </owl:NamedIndividual>
    


    <!-- http://purl.obolibrary.org/obo/GAZ_00027678 -->

    <owl:NamedIndividual rdf:about="http://purl.obolibrary.org/obo/GAZ_00027678">
        <obo:RO_0001025 rdf:resource="http://purl.obolibrary.org/obo/GAZ_02000765"/>
        <obo:IAO_0000115>A county of P&apos;yongan-nam Province.</obo:IAO_0000115>
        <oboInOwl:hasOBONamespace>GAZ</oboInOwl:hasOBONamespace>
        <oboInOwl:id>GAZ:00027678</oboInOwl:id>
        <rdfs:label>Hoech&apos;ang County</rdfs:label>
    </owl:NamedIndividual>
    


    <!-- http://purl.obolibrary.org/obo/GAZ_00027679 -->

    <owl:NamedIndividual rdf:about="http://purl.obolibrary.org/obo/GAZ_00027679">
        <obo:RO_0001025 rdf:resource="http://purl.obolibrary.org/obo/GAZ_02000765"/>
        <obo:IAO_0000115>A county of P&apos;yongan-nam Province.</obo:IAO_0000115>
        <oboInOwl:hasOBONamespace>GAZ</oboInOwl:hasOBONamespace>
        <oboInOwl:id>GAZ:00027679</oboInOwl:id>
        <rdfs:label>Songch&apos;on County</rdfs:label>
    </owl:NamedIndividual>
    


    <!-- http://purl.obolibrary.org/obo/GAZ_00027680 -->

    <owl:NamedIndividual rdf:about="http://purl.obolibrary.org/obo/GAZ_00027680">
        <obo:RO_0001025 rdf:resource="http://purl.obolibrary.org/obo/GAZ_02000765"/>
        <obo:IAO_0000115>A county of P&apos;yongan-nam Province.</obo:IAO_0000115>
        <oboInOwl:hasOBONamespace>GAZ</oboInOwl:hasOBONamespace>
        <oboInOwl:id>GAZ:00027680</oboInOwl:id>
        <rdfs:label>Taedong County</rdfs:label>
    </owl:NamedIndividual>
    


    <!-- http://purl.obolibrary.org/obo/GAZ_00027681 -->

    <owl:NamedIndividual rdf:about="http://purl.obolibrary.org/obo/GAZ_00027681">
        <obo:RO_0001025 rdf:resource="http://purl.obolibrary.org/obo/GAZ_02000765"/>
        <obo:IAO_0000115>A county of P&apos;yongan-nam Province.</obo:IAO_0000115>
        <oboInOwl:hasOBONamespace>GAZ</oboInOwl:hasOBONamespace>
        <oboInOwl:id>GAZ:00027681</oboInOwl:id>
        <rdfs:label>Chungsan County</rdfs:label>
    </owl:NamedIndividual>
    


    <!-- http://purl.obolibrary.org/obo/GAZ_00027682 -->

    <owl:NamedIndividual rdf:about="http://purl.obolibrary.org/obo/GAZ_00027682">
        <obo:RO_0001025 rdf:resource="http://purl.obolibrary.org/obo/GAZ_02000765"/>
        <obo:IAO_0000115>A county of P&apos;yongan-nam Province.</obo:IAO_0000115>
        <oboInOwl:hasOBONamespace>GAZ</oboInOwl:hasOBONamespace>
        <oboInOwl:id>GAZ:00027682</oboInOwl:id>
        <rdfs:label>Mundok County</rdfs:label>
    </owl:NamedIndividual>
    


    <!-- http://purl.obolibrary.org/obo/GAZ_00027683 -->

    <owl:NamedIndividual rdf:about="http://purl.obolibrary.org/obo/GAZ_00027683">
        <obo:RO_0001025 rdf:resource="http://purl.obolibrary.org/obo/GAZ_02000765"/>
        <obo:IAO_0000115>A county of P&apos;yongan-nam Province.</obo:IAO_0000115>
        <oboInOwl:hasOBONamespace>GAZ</oboInOwl:hasOBONamespace>
        <oboInOwl:id>GAZ:00027683</oboInOwl:id>
        <rdfs:label>Sinyang County</rdfs:label>
    </owl:NamedIndividual>
    


    <!-- http://purl.obolibrary.org/obo/GAZ_00027684 -->

    <owl:NamedIndividual rdf:about="http://purl.obolibrary.org/obo/GAZ_00027684">
        <obo:RO_0001025 rdf:resource="http://purl.obolibrary.org/obo/GAZ_02000765"/>
        <obo:IAO_0000115>A county of P&apos;yongan-nam Province.</obo:IAO_0000115>
        <oboInOwl:hasOBONamespace>GAZ</oboInOwl:hasOBONamespace>
        <oboInOwl:id>GAZ:00027684</oboInOwl:id>
        <rdfs:label>P&apos;yongwon County</rdfs:label>
    </owl:NamedIndividual>
    


    <!-- http://purl.obolibrary.org/obo/GAZ_00027685 -->

    <owl:NamedIndividual rdf:about="http://purl.obolibrary.org/obo/GAZ_00027685">
        <obo:RO_0001025 rdf:resource="http://purl.obolibrary.org/obo/GAZ_02000765"/>
        <obo:IAO_0000115>A county of P&apos;yongan-nam Province.</obo:IAO_0000115>
        <oboInOwl:hasOBONamespace>GAZ</oboInOwl:hasOBONamespace>
        <oboInOwl:id>GAZ:00027685</oboInOwl:id>
        <rdfs:label>Sukch&apos;on County</rdfs:label>
    </owl:NamedIndividual>
    


    <!-- http://purl.obolibrary.org/obo/GAZ_00027686 -->

    <owl:NamedIndividual rdf:about="http://purl.obolibrary.org/obo/GAZ_00027686">
        <obo:RO_0001025 rdf:resource="http://purl.obolibrary.org/obo/GAZ_02000762"/>
        <obo:IAO_0000115>A county in Ryanggang province, North Korea.</obo:IAO_0000115>
        <oboInOwl:hasOBONamespace>GAZ</oboInOwl:hasOBONamespace>
        <oboInOwl:id>GAZ:00027686</oboInOwl:id>
        <rdfs:label>Paegam County</rdfs:label>
    </owl:NamedIndividual>
    


    <!-- http://purl.obolibrary.org/obo/GAZ_00027687 -->

    <owl:NamedIndividual rdf:about="http://purl.obolibrary.org/obo/GAZ_00027687">
        <obo:RO_0001025 rdf:resource="http://purl.obolibrary.org/obo/GAZ_02000762"/>
        <obo:IAO_0000115>A populated place. A city in the northern part of the northern Ryanggang province of North Korea.</obo:IAO_0000115>
        <oboInOwl:hasOBONamespace>GAZ</oboInOwl:hasOBONamespace>
        <oboInOwl:id>GAZ:00027687</oboInOwl:id>
        <rdfs:label>Hyesan City</rdfs:label>
    </owl:NamedIndividual>
    


    <!-- http://purl.obolibrary.org/obo/GAZ_00027688 -->

    <owl:NamedIndividual rdf:about="http://purl.obolibrary.org/obo/GAZ_00027688">
        <obo:RO_0001025 rdf:resource="http://purl.obolibrary.org/obo/GAZ_02000760"/>
        <obo:IAO_0000115>A county in southeastern Chagang Province, North Korea. It borders Rangrim, Changjin, Chonchon, Tongsin, Taehung, and Songgan counties.</obo:IAO_0000115>
        <oboInOwl:hasOBONamespace>GAZ</oboInOwl:hasOBONamespace>
        <oboInOwl:id>GAZ:00027688</oboInOwl:id>
        <rdfs:label>Ryongrim County</rdfs:label>
    </owl:NamedIndividual>
    


    <!-- http://purl.obolibrary.org/obo/GAZ_00027689 -->

    <owl:NamedIndividual rdf:about="http://purl.obolibrary.org/obo/GAZ_00027689">
        <obo:RO_0001025 rdf:resource="http://purl.obolibrary.org/obo/GAZ_02000760"/>
        <obo:IAO_0000115>The provincial capital of Chagang Province, North Korea.</obo:IAO_0000115>
        <oboInOwl:hasOBONamespace>GAZ</oboInOwl:hasOBONamespace>
        <oboInOwl:id>GAZ:00027689</oboInOwl:id>
        <rdfs:label>Kanggye City</rdfs:label>
    </owl:NamedIndividual>
    


    <!-- http://purl.obolibrary.org/obo/GAZ_00027690 -->

    <owl:NamedIndividual rdf:about="http://purl.obolibrary.org/obo/GAZ_00027690">
        <obo:RO_0001025 rdf:resource="http://purl.obolibrary.org/obo/GAZ_02000760"/>
        <obo:IAO_0000115>A city of northwestern Chagang Province, North Korea.</obo:IAO_0000115>
        <oboInOwl:hasOBONamespace>GAZ</oboInOwl:hasOBONamespace>
        <oboInOwl:id>GAZ:00027690</oboInOwl:id>
        <rdfs:label>Manp&apos;o City</rdfs:label>
    </owl:NamedIndividual>
    


    <!-- http://purl.obolibrary.org/obo/GAZ_00027691 -->

    <owl:NamedIndividual rdf:about="http://purl.obolibrary.org/obo/GAZ_00027691">
        <obo:RO_0001025 rdf:resource="http://purl.obolibrary.org/obo/GAZ_02000760"/>
        <obo:IAO_0000115>A county in southwestern Chagang province, North Korea. It borders Usi and Kopung counties to the north, Tongsin to the east, and Huichon to the south, as well as North Pyongan&apos;s Tongchang county to the west. Originally part of Chosan, it was established as a separate county in 1949, when Chagang province was created.</obo:IAO_0000115>
        <oboInOwl:hasOBONamespace>GAZ</oboInOwl:hasOBONamespace>
        <oboInOwl:id>GAZ:00027691</oboInOwl:id>
        <rdfs:label>Songwon County</rdfs:label>
    </owl:NamedIndividual>
    


    <!-- http://purl.obolibrary.org/obo/GAZ_00027692 -->

    <owl:NamedIndividual rdf:about="http://purl.obolibrary.org/obo/GAZ_00027692">
        <obo:RO_0001025 rdf:resource="http://purl.obolibrary.org/obo/GAZ_02000760"/>
        <obo:IAO_0000115>A county in northern Chagang province, North Korea. It stands across the Yalu River from the People&apos;s Republic of China. It was originally part of North Pyongan province, but was annexed to Chagang in 1954. It borders Manpo and Sijungto the north, Kanggye and Songgan to the east, Chonchon to the southeast, Kopung to the south and west, and Chosan to the west.</obo:IAO_0000115>
        <oboInOwl:hasOBONamespace>GAZ</oboInOwl:hasOBONamespace>
        <oboInOwl:id>GAZ:00027692</oboInOwl:id>
        <rdfs:label>Wiwon County</rdfs:label>
    </owl:NamedIndividual>
    


    <!-- http://purl.obolibrary.org/obo/GAZ_00027693 -->

    <owl:NamedIndividual rdf:about="http://purl.obolibrary.org/obo/GAZ_00027693">
        <obo:RO_0001025 rdf:resource="http://purl.obolibrary.org/obo/GAZ_02000760"/>
        <obo:IAO_0000115>A county on the eastern flank of Chagang province, North Korea. It was created in 1952 from portions of Changgang and Changjin, as part of a general reorganization of local government. Originally part of South Hamgyong, it was transferred to Chagang province in 1954. It borders Hwapyong and Ryanggang&apos;s Kimjongsuk and Kimhyongjik counties to the north, South Hamgyong&apos;s Pujon county to the east and Changjin to the south, as well as the counties of Changgang, Songgan, and Yongrim to the west.</obo:IAO_0000115>
        <oboInOwl:hasOBONamespace>GAZ</oboInOwl:hasOBONamespace>
        <oboInOwl:id>GAZ:00027693</oboInOwl:id>
        <rdfs:label>Rangrim County</rdfs:label>
    </owl:NamedIndividual>
    


    <!-- http://purl.obolibrary.org/obo/GAZ_00027694 -->

    <owl:NamedIndividual rdf:about="http://purl.obolibrary.org/obo/GAZ_00027694">
        <obo:RO_0001025 rdf:resource="http://purl.obolibrary.org/obo/GAZ_02000760"/>
        <obo:IAO_0000115>A county in southern Chagang province, North Korea. It borders Ryongrim and Chonchon to the north, the counties of Taehung and Yongwon in South Pyongan to the south and east, and Huichon and Songwon to the west and southwest. Originally part of Huichon, it was created in 1952.</obo:IAO_0000115>
        <oboInOwl:hasOBONamespace>GAZ</oboInOwl:hasOBONamespace>
        <oboInOwl:id>GAZ:00027694</oboInOwl:id>
        <rdfs:label>Tongsin County</rdfs:label>
    </owl:NamedIndividual>
    


    <!-- http://purl.obolibrary.org/obo/GAZ_00027695 -->

    <owl:NamedIndividual rdf:about="http://purl.obolibrary.org/obo/GAZ_00027695">
        <obo:RO_0001025 rdf:resource="http://purl.obolibrary.org/obo/GAZ_02000760"/>
        <obo:IAO_0000115>A county in Chagang province, North Korea. It borders the People&apos;s Republic of China to the north.</obo:IAO_0000115>
        <oboInOwl:hasOBONamespace>GAZ</oboInOwl:hasOBONamespace>
        <oboInOwl:id>GAZ:00027695</oboInOwl:id>
        <rdfs:label>Ch&apos;osan County</rdfs:label>
    </owl:NamedIndividual>
    


    <!-- http://purl.obolibrary.org/obo/GAZ_00027696 -->

    <owl:NamedIndividual rdf:about="http://purl.obolibrary.org/obo/GAZ_00027696">
        <obo:RO_0001025 rdf:resource="http://purl.obolibrary.org/obo/GAZ_02000760"/>
        <obo:IAO_0000115>A county in westernmost Chagang province, North Korea. It looks across the Yalu River into the People&apos;s Republic of China. Within North Korea, it borders Chosan and Kopung to the east, Songwon to the south, and North Pyongan&apos;s Pyoktong county to the west. Originally part of Pyoktong, it was made a separate county in 1952; in 1954 it was transferred from North Pyongan to Chagang.</obo:IAO_0000115>
        <oboInOwl:hasOBONamespace>GAZ</oboInOwl:hasOBONamespace>
        <oboInOwl:id>GAZ:00027696</oboInOwl:id>
        <rdfs:label>Usi County</rdfs:label>
    </owl:NamedIndividual>
    


    <!-- http://purl.obolibrary.org/obo/GAZ_00027697 -->

    <owl:NamedIndividual rdf:about="http://purl.obolibrary.org/obo/GAZ_00027697">
        <obo:RO_0001025 rdf:resource="http://purl.obolibrary.org/obo/GAZ_02000760"/>
        <obo:IAO_0000115>A county in Chagang Province, North Korea.</obo:IAO_0000115>
        <oboInOwl:hasOBONamespace>GAZ</oboInOwl:hasOBONamespace>
        <oboInOwl:id>GAZ:00027697</oboInOwl:id>
        <rdfs:label>Chasong County</rdfs:label>
    </owl:NamedIndividual>
    


    <!-- http://purl.obolibrary.org/obo/GAZ_00027698 -->

    <owl:NamedIndividual rdf:about="http://purl.obolibrary.org/obo/GAZ_00027698">
        <obo:RO_0001025 rdf:resource="http://purl.obolibrary.org/obo/GAZ_02000760"/>
        <obo:IAO_0000115>A populated place. A city in the southern part of Chagang Province, North Korea.</obo:IAO_0000115>
        <oboInOwl:hasOBONamespace>GAZ</oboInOwl:hasOBONamespace>
        <oboInOwl:id>GAZ:00027698</oboInOwl:id>
        <rdfs:label>Huich&apos;on City</rdfs:label>
    </owl:NamedIndividual>
    


    <!-- http://purl.obolibrary.org/obo/GAZ_00027699 -->

    <owl:NamedIndividual rdf:about="http://purl.obolibrary.org/obo/GAZ_00027699">
        <obo:RO_0001025 rdf:resource="http://purl.obolibrary.org/obo/GAZ_02000760"/>
        <obo:IAO_0000115>A county in central Chagang province, North Korea. It borders Rangrim to the east, Wiwon to the west, Kanggye to the north and Chonchon and Ryongrim to the south. It was formed in 1952 from parts of Chonchon and Changgang.</obo:IAO_0000115>
        <oboInOwl:hasOBONamespace>GAZ</oboInOwl:hasOBONamespace>
        <oboInOwl:id>GAZ:00027699</oboInOwl:id>
        <rdfs:label>Songgan County</rdfs:label>
    </owl:NamedIndividual>
    


    <!-- http://purl.obolibrary.org/obo/GAZ_00027700 -->

    <owl:NamedIndividual rdf:about="http://purl.obolibrary.org/obo/GAZ_00027700">
        <obo:RO_0001025 rdf:resource="http://purl.obolibrary.org/obo/GAZ_02000760"/>
        <obo:IAO_0000115>A county in Chagang province, North Korea. It was incorporated as a new county in 1952-12. Previously it had been part of Chasong and Huchang.</obo:IAO_0000115>
        <oboInOwl:hasOBONamespace>GAZ</oboInOwl:hasOBONamespace>
        <oboInOwl:id>GAZ:00027700</oboInOwl:id>
        <rdfs:label>Hwap&apos;yong County</rdfs:label>
    </owl:NamedIndividual>
    


    <!-- http://purl.obolibrary.org/obo/GAZ_00027701 -->

    <owl:NamedIndividual rdf:about="http://purl.obolibrary.org/obo/GAZ_00027701">
        <obo:RO_0001025 rdf:resource="http://purl.obolibrary.org/obo/GAZ_02000760"/>
        <obo:IAO_0000115>A county, in central Chagang province, North Korea. Originally part of Kanggye, it was made a separate county in 1949.</obo:IAO_0000115>
        <oboInOwl:hasOBONamespace>GAZ</oboInOwl:hasOBONamespace>
        <oboInOwl:id>GAZ:00027701</oboInOwl:id>
        <rdfs:label>Chonch&apos;on County</rdfs:label>
    </owl:NamedIndividual>
    


    <!-- http://purl.obolibrary.org/obo/GAZ_00027702 -->

    <owl:NamedIndividual rdf:about="http://purl.obolibrary.org/obo/GAZ_00027702">
        <obo:RO_0001025 rdf:resource="http://purl.obolibrary.org/obo/GAZ_02000760"/>
        <oboInOwl:hasOBONamespace>GAZ</oboInOwl:hasOBONamespace>
        <oboInOwl:id>GAZ:00027702</oboInOwl:id>
        <rdfs:label>Changgang County</rdfs:label>
    </owl:NamedIndividual>
    


    <!-- http://purl.obolibrary.org/obo/GAZ_00027703 -->

    <owl:NamedIndividual rdf:about="http://purl.obolibrary.org/obo/GAZ_00027703">
        <obo:RO_0001025 rdf:resource="http://purl.obolibrary.org/obo/GAZ_02000760"/>
        <obo:IAO_0000115>A county in Chagang province, North Korea. It borders Kanggye and Changgang to the east, Manpo to the north and west, and Wiwon to the south. Formerly part of Kanggye, Sijung became a separate county in 1952.</obo:IAO_0000115>
        <oboInOwl:hasOBONamespace>GAZ</oboInOwl:hasOBONamespace>
        <oboInOwl:id>GAZ:00027703</oboInOwl:id>
        <rdfs:label>Sijung County</rdfs:label>
    </owl:NamedIndividual>
    


    <!-- http://purl.obolibrary.org/obo/GAZ_00027704 -->

    <owl:NamedIndividual rdf:about="http://purl.obolibrary.org/obo/GAZ_00027704">
        <obo:RO_0001025 rdf:resource="http://purl.obolibrary.org/obo/GAZ_02000760"/>
        <obo:IAO_0000115>A county in Chagang province, North Korea. Prior to the division of Korea, it was part of Chosan county.</obo:IAO_0000115>
        <oboInOwl:hasOBONamespace>GAZ</oboInOwl:hasOBONamespace>
        <oboInOwl:id>GAZ:00027704</oboInOwl:id>
        <rdfs:label>Kop&apos;ung County</rdfs:label>
    </owl:NamedIndividual>
    


    <!-- http://purl.obolibrary.org/obo/GAZ_00027705 -->

    <owl:NamedIndividual rdf:about="http://purl.obolibrary.org/obo/GAZ_00027705">
        <obo:RO_0001025 rdf:resource="http://purl.obolibrary.org/obo/GAZ_02000760"/>
        <obo:IAO_0000115>A county in northern Chagang province, North Korea. It was originally part of Huchang county in Ryanggang.</obo:IAO_0000115>
        <oboInOwl:hasOBONamespace>GAZ</oboInOwl:hasOBONamespace>
        <oboInOwl:id>GAZ:00027705</oboInOwl:id>
        <rdfs:label>Chunggang County</rdfs:label>
    </owl:NamedIndividual>
    


    <!-- http://purl.obolibrary.org/obo/GAZ_00027706 -->

    <owl:NamedIndividual rdf:about="http://purl.obolibrary.org/obo/GAZ_00027706">
        <obo:RO_0001025 rdf:resource="http://purl.obolibrary.org/obo/GAZ_00057403"/>
        <obo:RO_0001025 rdf:resource="http://purl.obolibrary.org/obo/GAZ_02000762"/>
        <obo:IAO_0000115>A county in Ryanggang province, North Korea. Kimhyongjik is located in the northwestern part of the Kaema Plateau. It borders China to the north (Yalu River region). Although the south is a plateau region, the Yalu River is in the north. The Huisaekbong Mountains and the Rangrim Mountains are partly in this county.</obo:IAO_0000115>
        <oboInOwl:hasOBONamespace>GAZ</oboInOwl:hasOBONamespace>
        <oboInOwl:id>GAZ:00027706</oboInOwl:id>
        <rdfs:label>Kimhyongjik County</rdfs:label>
    </owl:NamedIndividual>
    


    <!-- http://purl.obolibrary.org/obo/GAZ_00027707 -->

    <owl:NamedIndividual rdf:about="http://purl.obolibrary.org/obo/GAZ_00027707">
        <obo:RO_0001025 rdf:resource="http://purl.obolibrary.org/obo/GAZ_00057403"/>
        <obo:RO_0001025 rdf:resource="http://purl.obolibrary.org/obo/GAZ_02000762"/>
        <obo:IAO_0000115>A county in Ryanggang province, North Korea.</obo:IAO_0000115>
        <oboInOwl:hasOBONamespace>GAZ</oboInOwl:hasOBONamespace>
        <oboInOwl:id>GAZ:00027707</oboInOwl:id>
        <rdfs:label>P&apos;ungso County</rdfs:label>
    </owl:NamedIndividual>
    


    <!-- http://purl.obolibrary.org/obo/GAZ_00027708 -->

    <owl:NamedIndividual rdf:about="http://purl.obolibrary.org/obo/GAZ_00027708">
        <obo:RO_0001025 rdf:resource="http://purl.obolibrary.org/obo/GAZ_02000762"/>
        <obo:IAO_0000115>A county in Ryanggang province, North Korea. Originally part of Samsu, the county was made a separate entity in 1981.</obo:IAO_0000115>
        <oboInOwl:hasOBONamespace>GAZ</oboInOwl:hasOBONamespace>
        <oboInOwl:id>GAZ:00027708</oboInOwl:id>
        <rdfs:label>Kimjongsuk County</rdfs:label>
    </owl:NamedIndividual>
    


    <!-- http://purl.obolibrary.org/obo/GAZ_00027709 -->

    <owl:NamedIndividual rdf:about="http://purl.obolibrary.org/obo/GAZ_00027709">
        <obo:RO_0001025 rdf:resource="http://purl.obolibrary.org/obo/GAZ_02000762"/>
        <obo:IAO_0000115>A county in Ryanggang province, North Korea. It was created following the division of Korea from portions of Hyesan and Kapsan.</obo:IAO_0000115>
        <oboInOwl:hasOBONamespace>GAZ</oboInOwl:hasOBONamespace>
        <oboInOwl:id>GAZ:00027709</oboInOwl:id>
        <rdfs:label>Unhung County</rdfs:label>
    </owl:NamedIndividual>
    


    <!-- http://purl.obolibrary.org/obo/GAZ_00027710 -->

    <owl:NamedIndividual rdf:about="http://purl.obolibrary.org/obo/GAZ_00027710">
        <obo:RO_0001025 rdf:resource="http://purl.obolibrary.org/obo/GAZ_02000762"/>
        <obo:IAO_0000115>A county in Ryanggang province, North Korea.</obo:IAO_0000115>
        <oboInOwl:hasOBONamespace>GAZ</oboInOwl:hasOBONamespace>
        <oboInOwl:id>GAZ:00027710</oboInOwl:id>
        <rdfs:label>Samjiyon County</rdfs:label>
    </owl:NamedIndividual>
    


    <!-- http://purl.obolibrary.org/obo/GAZ_00027711 -->

    <owl:NamedIndividual rdf:about="http://purl.obolibrary.org/obo/GAZ_00027711">
        <obo:RO_0001025 rdf:resource="http://purl.obolibrary.org/obo/GAZ_02000762"/>
        <obo:IAO_0000115>A county in Ryanggang province, North Korea.</obo:IAO_0000115>
        <oboInOwl:hasOBONamespace>GAZ</oboInOwl:hasOBONamespace>
        <oboInOwl:id>GAZ:00027711</oboInOwl:id>
        <rdfs:label>Poch&apos;on County</rdfs:label>
    </owl:NamedIndividual>
    


    <!-- http://purl.obolibrary.org/obo/GAZ_00027712 -->

    <owl:NamedIndividual rdf:about="http://purl.obolibrary.org/obo/GAZ_00027712">
        <obo:RO_0001025 rdf:resource="http://purl.obolibrary.org/obo/GAZ_02000762"/>
        <obo:IAO_0000115>A county in Ryanggang province, North Korea. It was originally part of Musan.</obo:IAO_0000115>
        <oboInOwl:hasOBONamespace>GAZ</oboInOwl:hasOBONamespace>
        <oboInOwl:id>GAZ:00027712</oboInOwl:id>
        <rdfs:label>Taehongdan County</rdfs:label>
    </owl:NamedIndividual>
    


    <!-- http://purl.obolibrary.org/obo/GAZ_00027713 -->

    <owl:NamedIndividual rdf:about="http://purl.obolibrary.org/obo/GAZ_00027713">
        <obo:RO_0001025 rdf:resource="http://purl.obolibrary.org/obo/GAZ_00057403"/>
        <obo:RO_0001025 rdf:resource="http://purl.obolibrary.org/obo/GAZ_02000762"/>
        <obo:IAO_0000115>A county in Ryanggang province, North Korea. Prior to 1954, it was part of Hamgyong-nam Province. On its northern border, Samsu shares the Yalu River with China. It also shares a border with the province of North Pyongan. To the south, it occupies the northern tip of the Kaema Plateau.</obo:IAO_0000115>
        <oboInOwl:hasOBONamespace>GAZ</oboInOwl:hasOBONamespace>
        <oboInOwl:id>GAZ:00027713</oboInOwl:id>
        <rdfs:label>Samsu County</rdfs:label>
    </owl:NamedIndividual>
    


    <!-- http://purl.obolibrary.org/obo/GAZ_00027714 -->

    <owl:NamedIndividual rdf:about="http://purl.obolibrary.org/obo/GAZ_00027714">
        <obo:RO_0001025 rdf:resource="http://purl.obolibrary.org/obo/GAZ_00057403"/>
        <obo:RO_0001025 rdf:resource="http://purl.obolibrary.org/obo/GAZ_02000762"/>
        <obo:IAO_0000115>A county in Ryanggang province, North Korea. It borders Hamgyong-nam Province to the south. Kimhyonggwon lies on the southeastern edge of the Kaema Plateau.</obo:IAO_0000115>
        <oboInOwl:hasOBONamespace>GAZ</oboInOwl:hasOBONamespace>
        <oboInOwl:id>GAZ:00027714</oboInOwl:id>
        <rdfs:label>Kimhyonggwon County</rdfs:label>
    </owl:NamedIndividual>
    


    <!-- http://purl.obolibrary.org/obo/GAZ_00027716 -->

    <owl:NamedIndividual rdf:about="http://purl.obolibrary.org/obo/GAZ_00027716">
        <obo:RO_0001025 rdf:resource="http://purl.obolibrary.org/obo/GAZ_02000759"/>
        <obo:IAO_0000115>A county in P&apos;yongan-buk Province, North Korea, at the mouth of the Yalu River.</obo:IAO_0000115>
        <oboInOwl:hasOBONamespace>GAZ</oboInOwl:hasOBONamespace>
        <oboInOwl:id>GAZ:00027716</oboInOwl:id>
        <rdfs:label>Ryongch&apos;on County</rdfs:label>
    </owl:NamedIndividual>
    


    <!-- http://purl.obolibrary.org/obo/GAZ_00027717 -->

    <owl:NamedIndividual rdf:about="http://purl.obolibrary.org/obo/GAZ_00027717">
        <obo:RO_0001025 rdf:resource="http://purl.obolibrary.org/obo/GAZ_02000759"/>
        <obo:IAO_0000115>A populated place. A city in central P&apos;yongan-buk Province, North Korea. It borders Taegwan to the north, Taechon to the east, Kwaksan and Chongju to the south, and Chonma to the north.</obo:IAO_0000115>
        <oboInOwl:hasOBONamespace>GAZ</oboInOwl:hasOBONamespace>
        <oboInOwl:id>GAZ:00027717</oboInOwl:id>
        <rdfs:label>Kusong City</rdfs:label>
    </owl:NamedIndividual>
    


    <!-- http://purl.obolibrary.org/obo/GAZ_00027718 -->

    <owl:NamedIndividual rdf:about="http://purl.obolibrary.org/obo/GAZ_00027718">
        <obo:RO_0001025 rdf:resource="http://purl.obolibrary.org/obo/GAZ_02000759"/>
        <obo:IAO_0000115>A county in P&apos;yongan-buk Province, North Korea. It occupies the Cholsan Peninsula, which juts into the Yellow Sea. Cholsan borders Yomju and Tongrim to the north, and is bounded on all other sides by water. Part in Sinuiju Special Administrative Region.</obo:IAO_0000115>
        <oboInOwl:hasOBONamespace>GAZ</oboInOwl:hasOBONamespace>
        <oboInOwl:id>GAZ:00027718</oboInOwl:id>
        <rdfs:label>Ch&apos;olsan County</rdfs:label>
    </owl:NamedIndividual>
    


    <!-- http://purl.obolibrary.org/obo/GAZ_00027719 -->

    <owl:NamedIndividual rdf:about="http://purl.obolibrary.org/obo/GAZ_00027719">
        <obo:RO_0001025 rdf:resource="http://purl.obolibrary.org/obo/GAZ_02000759"/>
        <obo:IAO_0000115>A county in P&apos;yongan-buk Province, North Korea. It lies on the Yalu River, bordering the People&apos;s Republic of China to the north. Within North Korea, it borders Changsong to the east, Chonma and Taegwan to the south, and Uiju to the west.</obo:IAO_0000115>
        <oboInOwl:hasOBONamespace>GAZ</oboInOwl:hasOBONamespace>
        <oboInOwl:id>GAZ:00027719</oboInOwl:id>
        <rdfs:label>Sakchu County</rdfs:label>
    </owl:NamedIndividual>
    


    <!-- http://purl.obolibrary.org/obo/GAZ_00027720 -->

    <owl:NamedIndividual rdf:about="http://purl.obolibrary.org/obo/GAZ_00027720">
        <obo:RO_0001025 rdf:resource="http://purl.obolibrary.org/obo/GAZ_02000759"/>
        <obo:IAO_0000115>A county in P&apos;yongan-buk Province, North Korea. It borders Taechon to the north, Pakchon to the east and southeast, and Chongju to the north. To the south, it looks out on the Yellow Sea. Unjon was created in 1952 from portions of Pakchon and Chongju, and subsequently reorganized in 1954 and 1958.</obo:IAO_0000115>
        <oboInOwl:hasOBONamespace>GAZ</oboInOwl:hasOBONamespace>
        <oboInOwl:id>GAZ:00027720</oboInOwl:id>
        <rdfs:label>Unjon County</rdfs:label>
    </owl:NamedIndividual>
    


    <!-- http://purl.obolibrary.org/obo/GAZ_00027721 -->

    <owl:NamedIndividual rdf:about="http://purl.obolibrary.org/obo/GAZ_00027721">
        <obo:RO_0001025 rdf:resource="http://purl.obolibrary.org/obo/GAZ_02000759"/>
        <obo:IAO_0000115>A county in SE P&apos;yongan-buk Province, North Korea. It was created in 1952 from part of Nyongbyon county. It borders Nyongbyon on the west, Hyangsan and Unsan on the north, Yongwon on the east, and Kaechon and Tokchon cities to the south.</obo:IAO_0000115>
        <oboInOwl:hasOBONamespace>GAZ</oboInOwl:hasOBONamespace>
        <oboInOwl:id>GAZ:00027721</oboInOwl:id>
        <rdfs:label>Kujang County</rdfs:label>
    </owl:NamedIndividual>
    


    <!-- http://purl.obolibrary.org/obo/GAZ_00027722 -->

    <owl:NamedIndividual rdf:about="http://purl.obolibrary.org/obo/GAZ_00027722">
        <obo:RO_0001025 rdf:resource="http://purl.obolibrary.org/obo/GAZ_02000759"/>
        <obo:IAO_0000115>A county in NW P&apos;yongan-buk Province, North Korea. It is bounded to the north by Uiju, to the east by Chonma, to the south by Yomju and Tongrim, and to the west by Ryongchon and the large city of Sinuiju. It was established as a separate county in 1952.</obo:IAO_0000115>
        <oboInOwl:hasOBONamespace>GAZ</oboInOwl:hasOBONamespace>
        <oboInOwl:id>GAZ:00027722</oboInOwl:id>
        <rdfs:label>P&apos;ihyon County</rdfs:label>
    </owl:NamedIndividual>
    


    <!-- http://purl.obolibrary.org/obo/GAZ_00027723 -->

    <owl:NamedIndividual rdf:about="http://purl.obolibrary.org/obo/GAZ_00027723">
        <obo:RO_0001025 rdf:resource="http://purl.obolibrary.org/obo/GAZ_02000759"/>
        <obo:IAO_0000115>A city, in southern P&apos;yongan-buk Province, North Korea. Chongju also includes approximately 10 islands in the Yellow Sea.</obo:IAO_0000115>
        <oboInOwl:hasOBONamespace>GAZ</oboInOwl:hasOBONamespace>
        <oboInOwl:id>GAZ:00027723</oboInOwl:id>
        <rdfs:label>Chongju City</rdfs:label>
    </owl:NamedIndividual>
    


    <!-- http://purl.obolibrary.org/obo/GAZ_00027724 -->

    <owl:NamedIndividual rdf:about="http://purl.obolibrary.org/obo/GAZ_00027724">
        <obo:RO_0001025 rdf:resource="http://purl.obolibrary.org/obo/GAZ_02000759"/>
        <obo:IAO_0000115>A county in P&apos;yongan-buk Province, North Korea. It borders Taegwan and Tongchang to the north, Unsan and Nyongbyon to the east, Pakchon and Unjon to the south, and Kusong to the west.</obo:IAO_0000115>
        <oboInOwl:hasOBONamespace>GAZ</oboInOwl:hasOBONamespace>
        <oboInOwl:id>GAZ:00027724</oboInOwl:id>
        <rdfs:label>T&apos;aech&apos;on County</rdfs:label>
    </owl:NamedIndividual>
    


    <!-- http://purl.obolibrary.org/obo/GAZ_00027725 -->

    <owl:NamedIndividual rdf:about="http://purl.obolibrary.org/obo/GAZ_00027725">
        <obo:RO_0001025 rdf:resource="http://purl.obolibrary.org/obo/GAZ_02000759"/>
        <obo:IAO_0000115>A county in S P&apos;yongan-buk Province, North Korea. It faces the Yellow Sea to the south. By land, it is bordered by Kusong in the north, Chongju in the east, and Sonchon in the west.</obo:IAO_0000115>
        <oboInOwl:hasOBONamespace>GAZ</oboInOwl:hasOBONamespace>
        <oboInOwl:id>GAZ:00027725</oboInOwl:id>
        <rdfs:label>Kwaksan County</rdfs:label>
    </owl:NamedIndividual>
    


    <!-- http://purl.obolibrary.org/obo/GAZ_00027726 -->

    <owl:NamedIndividual rdf:about="http://purl.obolibrary.org/obo/GAZ_00027726">
        <obo:RO_0001025 rdf:resource="http://purl.obolibrary.org/obo/GAZ_02000759"/>
        <obo:IAO_0000115>A county in P&apos;yongan-buk Province, North Korea. It lies in the valley of the Yalu River, and borders China to the north. Within North Korea, it is bounded by Tongchang in the south, Changsong in the west, and Usi county in Chagang province to the east. It was separated from Usi in 1952.</obo:IAO_0000115>
        <oboInOwl:hasOBONamespace>GAZ</oboInOwl:hasOBONamespace>
        <oboInOwl:id>GAZ:00027726</oboInOwl:id>
        <rdfs:label>Pyoktong County</rdfs:label>
    </owl:NamedIndividual>
    


    <!-- http://purl.obolibrary.org/obo/GAZ_00027727 -->

    <owl:NamedIndividual rdf:about="http://purl.obolibrary.org/obo/GAZ_00027727">
        <obo:RO_0001025 rdf:resource="http://purl.obolibrary.org/obo/GAZ_00027637"/>
        <obo:RO_0001025 rdf:resource="http://purl.obolibrary.org/obo/GAZ_02000759"/>
        <obo:IAO_0000115>A populated place. A city in North Korea, on the border with China and is the capital of P&apos;yongan-buk Province. Part of the city is included in the Sinuiju Special Administrative Region, which was established in 2002. The border with China is marked by the Yalu (Amnok) River. The city is connected to Dandong in China via the Sino-Korea Friendship Bridge (or China-Korea Friendship Bridge). Part in the Sinuiju Special Administrative Region.</obo:IAO_0000115>
        <oboInOwl:hasOBONamespace>GAZ</oboInOwl:hasOBONamespace>
        <oboInOwl:id>GAZ:00027727</oboInOwl:id>
        <rdfs:label>Sinuiju City</rdfs:label>
    </owl:NamedIndividual>
    


    <!-- http://purl.obolibrary.org/obo/GAZ_00027728 -->

    <owl:NamedIndividual rdf:about="http://purl.obolibrary.org/obo/GAZ_00027728">
        <obo:RO_0001025 rdf:resource="http://purl.obolibrary.org/obo/GAZ_02000759"/>
        <obo:IAO_0000115>A county in P&apos;yongan-buk Province, North Korea. Most of the county consists of Pidansom, an island in the estuary of the Yalu River. Sindo was established as a separate county in 1991; previously, it had been part of Ryongchon, although it had enjoyed a brief existence as a separate county in 1967.</obo:IAO_0000115>
        <oboInOwl:hasOBONamespace>GAZ</oboInOwl:hasOBONamespace>
        <oboInOwl:id>GAZ:00027728</oboInOwl:id>
        <rdfs:label>Sindo County</rdfs:label>
    </owl:NamedIndividual>
    


    <!-- http://purl.obolibrary.org/obo/GAZ_00027729 -->

    <owl:NamedIndividual rdf:about="http://purl.obolibrary.org/obo/GAZ_00027729">
        <obo:RO_0001025 rdf:resource="http://purl.obolibrary.org/obo/GAZ_02000759"/>
        <obo:IAO_0000115>A county in P&apos;yongan-buk Province, North Korea. It borders Kusong and Taegwan to the east, Sonchon and Tongrim to the south, Uiju and Pihyon to the west, and Sakchu to the north. It was created in 1952 from parts of Kusong and Uiju.</obo:IAO_0000115>
        <oboInOwl:hasOBONamespace>GAZ</oboInOwl:hasOBONamespace>
        <oboInOwl:id>GAZ:00027729</oboInOwl:id>
        <rdfs:label>Ch&apos;onma County</rdfs:label>
    </owl:NamedIndividual>
    


    <!-- http://purl.obolibrary.org/obo/GAZ_00027730 -->

    <owl:NamedIndividual rdf:about="http://purl.obolibrary.org/obo/GAZ_00027730">
        <obo:RO_0001025 rdf:resource="http://purl.obolibrary.org/obo/GAZ_02000759"/>
        <obo:IAO_0000115>A county in P&apos;yongan-buk Province, North Korea. It lies in the province&apos;s interior, and is bounded by Tongchang on the east, Kusong and Taechon to the south, Chonma to the west, and Changsong and Sakchu to the north. It was created in 1952 from portions of Sakchu county.</obo:IAO_0000115>
        <oboInOwl:hasOBONamespace>GAZ</oboInOwl:hasOBONamespace>
        <oboInOwl:id>GAZ:00027730</oboInOwl:id>
        <rdfs:label>Taegwan County</rdfs:label>
    </owl:NamedIndividual>
    


    <!-- http://purl.obolibrary.org/obo/GAZ_00027731 -->

    <owl:NamedIndividual rdf:about="http://purl.obolibrary.org/obo/GAZ_00027731">
        <obo:RO_0001025 rdf:resource="http://purl.obolibrary.org/obo/GAZ_02000759"/>
        <obo:IAO_0000115>A county in P&apos;yongan-buk Province, North Korea. It borders the cities of Kaech&apos;on and Anju.</obo:IAO_0000115>
        <oboInOwl:hasOBONamespace>GAZ</oboInOwl:hasOBONamespace>
        <oboInOwl:id>GAZ:00027731</oboInOwl:id>
        <rdfs:label>Nyongbyon County</rdfs:label>
    </owl:NamedIndividual>
    


    <!-- http://purl.obolibrary.org/obo/GAZ_00027732 -->

    <owl:NamedIndividual rdf:about="http://purl.obolibrary.org/obo/GAZ_00027732">
        <obo:RO_0001025 rdf:resource="http://purl.obolibrary.org/obo/GAZ_02000759"/>
        <obo:IAO_0000115>A county in P&apos;yongan-buk Province, North Korea. To the north it borders Chonma, to the east Kusong and Kwaksan, and to the west Tongrim; to the south, it borders nothing but the sea. Sonchon was reorganized in 1952, with two myeon, or townships, being split off to form the new county of Tongrim.</obo:IAO_0000115>
        <oboInOwl:hasOBONamespace>GAZ</oboInOwl:hasOBONamespace>
        <oboInOwl:id>GAZ:00027732</oboInOwl:id>
        <rdfs:label>Sonch&apos;on County</rdfs:label>
    </owl:NamedIndividual>
    


    <!-- http://purl.obolibrary.org/obo/GAZ_00027733 -->

    <owl:NamedIndividual rdf:about="http://purl.obolibrary.org/obo/GAZ_00027733">
        <obo:RO_0001025 rdf:resource="http://purl.obolibrary.org/obo/GAZ_02000759"/>
        <obo:IAO_0000115>A county in P&apos;yongan-buk Province, North Korea. It was established, following the division of Korea, from portions of Nyongbyon county.</obo:IAO_0000115>
        <oboInOwl:hasOBONamespace>GAZ</oboInOwl:hasOBONamespace>
        <oboInOwl:id>GAZ:00027733</oboInOwl:id>
        <rdfs:label>Hyangsan County</rdfs:label>
    </owl:NamedIndividual>
    


    <!-- http://purl.obolibrary.org/obo/GAZ_00027734 -->

    <owl:NamedIndividual rdf:about="http://purl.obolibrary.org/obo/GAZ_00027734">
        <obo:RO_0001025 rdf:resource="http://purl.obolibrary.org/obo/GAZ_02000759"/>
        <obo:IAO_0000115>A county in P&apos;yongan-buk Province, North Korea. It borders Hyangsan in the east, Kujang and Nyongbyon in the south, and Tongchang and Taechon in the west. In addition, it is bordered by Chagang province to the east (Huichon) and north (Songwon).</obo:IAO_0000115>
        <oboInOwl:hasOBONamespace>GAZ</oboInOwl:hasOBONamespace>
        <oboInOwl:id>GAZ:00027734</oboInOwl:id>
        <rdfs:label>Unsan County</rdfs:label>
    </owl:NamedIndividual>
    


    <!-- http://purl.obolibrary.org/obo/GAZ_00027735 -->

    <owl:NamedIndividual rdf:about="http://purl.obolibrary.org/obo/GAZ_00027735">
        <obo:RO_0001025 rdf:resource="http://purl.obolibrary.org/obo/GAZ_02000759"/>
        <obo:IAO_0000115>A county in P&apos;yongan-buk Province, North Korea. It is bordered by Ryongchon and Pihyon to the north, Tongrim to the east, and Cholsan to the south; to the west lies the Yellow Sea. The county was created in 1952 from portions of Cholsan and Ryongchon. Part in Sinuiju Special Administrative Region.</obo:IAO_0000115>
        <oboInOwl:hasOBONamespace>GAZ</oboInOwl:hasOBONamespace>
        <oboInOwl:id>GAZ:00027735</oboInOwl:id>
        <rdfs:label>Yomju County</rdfs:label>
    </owl:NamedIndividual>
    


    <!-- http://purl.obolibrary.org/obo/GAZ_00027736 -->

    <owl:NamedIndividual rdf:about="http://purl.obolibrary.org/obo/GAZ_00027736">
        <obo:RO_0001025 rdf:resource="http://purl.obolibrary.org/obo/GAZ_02000759"/>
        <obo:IAO_0000115>A county in P&apos;yongan-buk Province, North Korea. It borders Pyoktong and Chagang&apos;s Usi county to the north, Unsan and Songwon to the east, Taechon to the south, and Changsong and Taegwan to the west.</obo:IAO_0000115>
        <oboInOwl:hasOBONamespace>GAZ</oboInOwl:hasOBONamespace>
        <oboInOwl:id>GAZ:00027736</oboInOwl:id>
        <rdfs:label>Tongch&apos;ang County</rdfs:label>
    </owl:NamedIndividual>
    


    <!-- http://purl.obolibrary.org/obo/GAZ_00027737 -->

    <owl:NamedIndividual rdf:about="http://purl.obolibrary.org/obo/GAZ_00027737">
        <obo:RO_0001025 rdf:resource="http://purl.obolibrary.org/obo/GAZ_02000759"/>
        <obo:IAO_0000115>A county in S P&apos;yongan-buk Province, North Korea. It is bordered to the north by Taechon, to the east and southeast by Nyongbyon, and to the west by Unjon. To the south, it looks across the Chongchon River at Anju city and Mudok county in South Pyongan province.</obo:IAO_0000115>
        <oboInOwl:hasOBONamespace>GAZ</oboInOwl:hasOBONamespace>
        <oboInOwl:id>GAZ:00027737</oboInOwl:id>
        <rdfs:label>Pakch&apos;on County</rdfs:label>
    </owl:NamedIndividual>
    


    <!-- http://purl.obolibrary.org/obo/GAZ_00027738 -->

    <owl:NamedIndividual rdf:about="http://purl.obolibrary.org/obo/GAZ_00027738">
        <obo:RO_0001025 rdf:resource="http://purl.obolibrary.org/obo/GAZ_02000759"/>
        <obo:IAO_0000115>A county in P&apos;yongan-buk Province, North Korea. It borders Pihyon and Chonma to the north, Sonchon to the east, Cholsan to the southwest, and Yomju to the west. To the south, it looks out on the Yellow Sea.</obo:IAO_0000115>
        <oboInOwl:hasOBONamespace>GAZ</oboInOwl:hasOBONamespace>
        <oboInOwl:id>GAZ:00027738</oboInOwl:id>
        <rdfs:label>Tongrim County</rdfs:label>
    </owl:NamedIndividual>
    


    <!-- http://purl.obolibrary.org/obo/GAZ_00027739 -->

    <owl:NamedIndividual rdf:about="http://purl.obolibrary.org/obo/GAZ_00027739">
        <obo:RO_0001025 rdf:resource="http://purl.obolibrary.org/obo/GAZ_02000759"/>
        <obo:IAO_0000115>A county in northern P&apos;yongan-buk Province, North Korea. It is bordered by Pyoktong to the east, Tongchang and Taegwan to the south, Sakchu to the west; to the north, it faces China across the Yalu River.</obo:IAO_0000115>
        <oboInOwl:hasOBONamespace>GAZ</oboInOwl:hasOBONamespace>
        <oboInOwl:id>GAZ:00027739</oboInOwl:id>
        <rdfs:label>Ch&apos;angsong County</rdfs:label>
    </owl:NamedIndividual>
    


    <!-- http://purl.obolibrary.org/obo/GAZ_00027740 -->

    <owl:NamedIndividual rdf:about="http://purl.obolibrary.org/obo/GAZ_00027740">
        <obo:RO_0001025 rdf:resource="http://purl.obolibrary.org/obo/GAZ_02000764"/>
        <obo:IAO_0000115>A county of Hwanghae-buk Province.</obo:IAO_0000115>
        <oboInOwl:hasOBONamespace>GAZ</oboInOwl:hasOBONamespace>
        <oboInOwl:id>GAZ:00027740</oboInOwl:id>
        <rdfs:label>Yonsan County</rdfs:label>
    </owl:NamedIndividual>
    


    <!-- http://purl.obolibrary.org/obo/GAZ_00027741 -->

    <owl:NamedIndividual rdf:about="http://purl.obolibrary.org/obo/GAZ_00027741">
        <obo:RO_0001025 rdf:resource="http://purl.obolibrary.org/obo/GAZ_02000761"/>
        <obo:IAO_0000115>A county of Hwanghae-nam Province, North Korea.</obo:IAO_0000115>
        <oboInOwl:hasOBONamespace>GAZ</oboInOwl:hasOBONamespace>
        <oboInOwl:id>GAZ:00027741</oboInOwl:id>
        <rdfs:label>Unryul County</rdfs:label>
    </owl:NamedIndividual>
    


    <!-- http://purl.obolibrary.org/obo/GAZ_00027742 -->

    <owl:NamedIndividual rdf:about="http://purl.obolibrary.org/obo/GAZ_00027742">
        <obo:RO_0001025 rdf:resource="http://purl.obolibrary.org/obo/GAZ_02000758"/>
        <obo:IAO_0000115>A port city and naval base in southeastern North Korea. It is the capital of Kangwon Province. It is located in Kangwon Province, on the westernmost part of the Sea of Japan (East Sea of Korea) and the east end of the Korean peninsula&apos;s neck.</obo:IAO_0000115>
        <oboInOwl:hasOBONamespace>GAZ</oboInOwl:hasOBONamespace>
        <oboInOwl:id>GAZ:00027742</oboInOwl:id>
        <rdfs:label>Wonsan City</rdfs:label>
    </owl:NamedIndividual>
    


    <!-- http://purl.obolibrary.org/obo/GAZ_00027743 -->

    <owl:NamedIndividual rdf:about="http://purl.obolibrary.org/obo/GAZ_00027743">
        <obo:RO_0001025 rdf:resource="http://purl.obolibrary.org/obo/GAZ_02000761"/>
        <obo:IAO_0000115>A city located in Hwanghae-nam Province near Haeju Bay in North Korea. It is the administrative centre of South Hwanghae Province.</obo:IAO_0000115>
        <oboInOwl:hasOBONamespace>GAZ</oboInOwl:hasOBONamespace>
        <oboInOwl:id>GAZ:00027743</oboInOwl:id>
        <rdfs:label>Haeju City</rdfs:label>
    </owl:NamedIndividual>
    


    <!-- http://purl.obolibrary.org/obo/GAZ_00027744 -->

    <owl:NamedIndividual rdf:about="http://purl.obolibrary.org/obo/GAZ_00027744">
        <obo:RO_0001025 rdf:resource="http://purl.obolibrary.org/obo/GAZ_02000761"/>
        <obo:IAO_0000115>A county of Hwanghae-nam Province, North Korea.</obo:IAO_0000115>
        <oboInOwl:hasOBONamespace>GAZ</oboInOwl:hasOBONamespace>
        <oboInOwl:id>GAZ:00027744</oboInOwl:id>
        <rdfs:label>Unch&apos;on County</rdfs:label>
    </owl:NamedIndividual>
    


    <!-- http://purl.obolibrary.org/obo/GAZ_00027745 -->

    <owl:NamedIndividual rdf:about="http://purl.obolibrary.org/obo/GAZ_00027745">
        <obo:RO_0001025 rdf:resource="http://purl.obolibrary.org/obo/GAZ_02000758"/>
        <obo:IAO_0000115>A county in Kangwon Province, North Korea.</obo:IAO_0000115>
        <oboInOwl:hasOBONamespace>GAZ</oboInOwl:hasOBONamespace>
        <oboInOwl:id>GAZ:00027745</oboInOwl:id>
        <rdfs:label>Kimhwa County</rdfs:label>
    </owl:NamedIndividual>
    


    <!-- http://purl.obolibrary.org/obo/GAZ_00027746 -->

    <owl:NamedIndividual rdf:about="http://purl.obolibrary.org/obo/GAZ_00027746">
        <obo:RO_0001025 rdf:resource="http://purl.obolibrary.org/obo/GAZ_02000758"/>
        <obo:IAO_0000115>A county in Kangwon Province, North Korea.</obo:IAO_0000115>
        <oboInOwl:hasOBONamespace>GAZ</oboInOwl:hasOBONamespace>
        <oboInOwl:id>GAZ:00027746</oboInOwl:id>
        <rdfs:label>Sep&apos;o County</rdfs:label>
    </owl:NamedIndividual>
    


    <!-- http://purl.obolibrary.org/obo/GAZ_00027747 -->

    <owl:NamedIndividual rdf:about="http://purl.obolibrary.org/obo/GAZ_00027747">
        <obo:RO_0001025 rdf:resource="http://purl.obolibrary.org/obo/GAZ_02000758"/>
        <obo:IAO_0000115>A county in Kangwon Province, North Korea. In 1952-12 P&apos;an&apos;gyo was formed as a separate county from five myon (Nagyang, Pangjang, P&apos;an&apos;gyo, Ryongp&apos;o, Sannae) of Ichon-gun and Yujin-myon of P&apos;yonggang-gun.</obo:IAO_0000115>
        <oboInOwl:hasOBONamespace>GAZ</oboInOwl:hasOBONamespace>
        <oboInOwl:id>GAZ:00027747</oboInOwl:id>
        <rdfs:label>P&apos;an&apos;gyo County</rdfs:label>
    </owl:NamedIndividual>
    


    <!-- http://purl.obolibrary.org/obo/GAZ_00027748 -->

    <owl:NamedIndividual rdf:about="http://purl.obolibrary.org/obo/GAZ_00027748">
        <obo:RO_0001025 rdf:resource="http://purl.obolibrary.org/obo/GAZ_02000758"/>
        <obo:IAO_0000115>A North Korean city located in Kangwon Province. It lies on the coast of the Sea of Japan. Munch&apos;on sits on Yonghung Bay, a bay of the Sea of Japan.</obo:IAO_0000115>
        <oboInOwl:hasOBONamespace>GAZ</oboInOwl:hasOBONamespace>
        <oboInOwl:id>GAZ:00027748</oboInOwl:id>
        <rdfs:label>Munch&apos;on City</rdfs:label>
    </owl:NamedIndividual>
    


    <!-- http://purl.obolibrary.org/obo/GAZ_00027749 -->

    <owl:NamedIndividual rdf:about="http://purl.obolibrary.org/obo/GAZ_00027749">
        <obo:RO_0001025 rdf:resource="http://purl.obolibrary.org/obo/GAZ_02000758"/>
        <obo:IAO_0000115>A county in northern Kangwon Province, North Korea. The county&apos;s borders run along the Masikryong and Ryongam ranges.</obo:IAO_0000115>
        <oboInOwl:hasOBONamespace>GAZ</oboInOwl:hasOBONamespace>
        <oboInOwl:id>GAZ:00027749</oboInOwl:id>
        <rdfs:label>Ich&apos;on County</rdfs:label>
    </owl:NamedIndividual>
    


    <!-- http://purl.obolibrary.org/obo/GAZ_00027750 -->

    <owl:NamedIndividual rdf:about="http://purl.obolibrary.org/obo/GAZ_00027750">
        <obo:RO_0001025 rdf:resource="http://purl.obolibrary.org/obo/GAZ_02000758"/>
        <obo:IAO_0000115>A county in Kangwon Province, North Korea. It lies in the southeasternmost corner of North Korea, immediately north of the Korean Demilitarized Zone. Prior to the end of the Korean War in 1953, it made up a single county, together with what is now the South Korean county of the same name. In a subsequent reorganization, the county absorbed the southern portion of Tongchon county.</obo:IAO_0000115>
        <oboInOwl:hasOBONamespace>GAZ</oboInOwl:hasOBONamespace>
        <oboInOwl:id>GAZ:00027750</oboInOwl:id>
        <rdfs:label>Kosong County</rdfs:label>
    </owl:NamedIndividual>
    


    <!-- http://purl.obolibrary.org/obo/GAZ_00027751 -->

    <owl:NamedIndividual rdf:about="http://purl.obolibrary.org/obo/GAZ_00027751">
        <obo:RO_0001025 rdf:resource="http://purl.obolibrary.org/obo/GAZ_02000761"/>
        <obo:IAO_0000115>A county of Hwanghae-nam Province, North Korea.</obo:IAO_0000115>
        <oboInOwl:hasOBONamespace>GAZ</oboInOwl:hasOBONamespace>
        <oboInOwl:id>GAZ:00027751</oboInOwl:id>
        <rdfs:label>Songhwa County</rdfs:label>
    </owl:NamedIndividual>
    


    <!-- http://purl.obolibrary.org/obo/GAZ_00027752 -->

    <owl:NamedIndividual rdf:about="http://purl.obolibrary.org/obo/GAZ_00027752">
        <obo:RO_0001025 rdf:resource="http://purl.obolibrary.org/obo/GAZ_02000758"/>
        <obo:IAO_0000115>A county in Kangwon Province, North Korea. It borders Sepo to the north, Chorwon to the south, Ichon to the west, and Changdo to the east.</obo:IAO_0000115>
        <oboInOwl:hasOBONamespace>GAZ</oboInOwl:hasOBONamespace>
        <oboInOwl:id>GAZ:00027752</oboInOwl:id>
        <rdfs:label>P&apos;yonggang County</rdfs:label>
    </owl:NamedIndividual>
    


    <!-- http://purl.obolibrary.org/obo/GAZ_00027753 -->

    <owl:NamedIndividual rdf:about="http://purl.obolibrary.org/obo/GAZ_00027753">
        <obo:RO_0001025 rdf:resource="http://purl.obolibrary.org/obo/GAZ_02000761"/>
        <obo:IAO_0000115>A county of Hwanghae-nam Province, North Korea.</obo:IAO_0000115>
        <oboInOwl:hasOBONamespace>GAZ</oboInOwl:hasOBONamespace>
        <oboInOwl:id>GAZ:00027753</oboInOwl:id>
        <rdfs:label>Sinwon County</rdfs:label>
    </owl:NamedIndividual>
    


    <!-- http://purl.obolibrary.org/obo/GAZ_00027754 -->

    <owl:NamedIndividual rdf:about="http://purl.obolibrary.org/obo/GAZ_00027754">
        <obo:RO_0001025 rdf:resource="http://purl.obolibrary.org/obo/GAZ_02000758"/>
        <obo:IAO_0000115>A county in Kangwon Province, North Korea. It abuts the Sea of Japan (East Sea of Korea) to the north and east.</obo:IAO_0000115>
        <oboInOwl:hasOBONamespace>GAZ</oboInOwl:hasOBONamespace>
        <oboInOwl:id>GAZ:00027754</oboInOwl:id>
        <rdfs:label>T&apos;ongch&apos;on County</rdfs:label>
    </owl:NamedIndividual>
    


    <!-- http://purl.obolibrary.org/obo/GAZ_00027755 -->

    <owl:NamedIndividual rdf:about="http://purl.obolibrary.org/obo/GAZ_00027755">
        <obo:RO_0001025 rdf:resource="http://purl.obolibrary.org/obo/GAZ_02000758"/>
        <obo:IAO_0000115>A county in Kangwon Province, North Korea.</obo:IAO_0000115>
        <oboInOwl:hasOBONamespace>GAZ</oboInOwl:hasOBONamespace>
        <oboInOwl:id>GAZ:00027755</oboInOwl:id>
        <rdfs:label>Kosan County</rdfs:label>
    </owl:NamedIndividual>
    


    <!-- http://purl.obolibrary.org/obo/GAZ_00027756 -->

    <owl:NamedIndividual rdf:about="http://purl.obolibrary.org/obo/GAZ_00027756">
        <obo:RO_0001025 rdf:resource="http://purl.obolibrary.org/obo/GAZ_02000758"/>
        <obo:IAO_0000115>A county in Kangwon Province, North Korea.</obo:IAO_0000115>
        <oboInOwl:hasOBONamespace>GAZ</oboInOwl:hasOBONamespace>
        <oboInOwl:id>GAZ:00027756</oboInOwl:id>
        <rdfs:label>Poptong County</rdfs:label>
    </owl:NamedIndividual>
    


    <!-- http://purl.obolibrary.org/obo/GAZ_00027757 -->

    <owl:NamedIndividual rdf:about="http://purl.obolibrary.org/obo/GAZ_00027757">
        <obo:RO_0001025 rdf:resource="http://purl.obolibrary.org/obo/GAZ_02000758"/>
        <obo:IAO_0000115>A county in Kangwon Province, North Korea. Established 1952.</obo:IAO_0000115>
        <oboInOwl:hasOBONamespace>GAZ</oboInOwl:hasOBONamespace>
        <oboInOwl:id>GAZ:00027757</oboInOwl:id>
        <rdfs:label>Hoeyang County</rdfs:label>
    </owl:NamedIndividual>
    


    <!-- http://purl.obolibrary.org/obo/GAZ_00027758 -->

    <owl:NamedIndividual rdf:about="http://purl.obolibrary.org/obo/GAZ_00027758">
        <obo:RO_0001025 rdf:resource="http://purl.obolibrary.org/obo/GAZ_02000758"/>
        <obo:IAO_0000115>A county in Kangwon Province, North Korea.</obo:IAO_0000115>
        <oboInOwl:hasOBONamespace>GAZ</oboInOwl:hasOBONamespace>
        <oboInOwl:id>GAZ:00027758</oboInOwl:id>
        <rdfs:label>Ch&apos;orwon County</rdfs:label>
    </owl:NamedIndividual>
    


    <!-- http://purl.obolibrary.org/obo/GAZ_00027759 -->

    <owl:NamedIndividual rdf:about="http://purl.obolibrary.org/obo/GAZ_00027759">
        <obo:RO_0001025 rdf:resource="http://purl.obolibrary.org/obo/GAZ_02000761"/>
        <obo:IAO_0000115>A county of Hwanghae-nam Province, North Korea.</obo:IAO_0000115>
        <oboInOwl:hasOBONamespace>GAZ</oboInOwl:hasOBONamespace>
        <oboInOwl:id>GAZ:00027759</oboInOwl:id>
        <rdfs:label>Yonan County</rdfs:label>
    </owl:NamedIndividual>
    


    <!-- http://purl.obolibrary.org/obo/GAZ_00027760 -->

    <owl:NamedIndividual rdf:about="http://purl.obolibrary.org/obo/GAZ_00027760">
        <obo:RO_0001025 rdf:resource="http://purl.obolibrary.org/obo/GAZ_02000758"/>
        <obo:IAO_0000115>A county, in Kangwon Province, North Korea. Originally included in Hamgyong-nam Province, it was transferred to Kangwon province in 1946-09. The southwest portion of the county is bounded by the Masikryong and Taebaek mountains, which meet at the pass of Chugaryong.</obo:IAO_0000115>
        <oboInOwl:hasOBONamespace>GAZ</oboInOwl:hasOBONamespace>
        <oboInOwl:id>GAZ:00027760</oboInOwl:id>
        <rdfs:label>Anbyon County</rdfs:label>
    </owl:NamedIndividual>
    


    <!-- http://purl.obolibrary.org/obo/GAZ_00027761 -->

    <owl:NamedIndividual rdf:about="http://purl.obolibrary.org/obo/GAZ_00027761">
        <obo:RO_0001025 rdf:resource="http://purl.obolibrary.org/obo/GAZ_02000761"/>
        <obo:IAO_0000115>A county of Hwanghae-nam Province, North Korea.</obo:IAO_0000115>
        <oboInOwl:hasOBONamespace>GAZ</oboInOwl:hasOBONamespace>
        <oboInOwl:id>GAZ:00027761</oboInOwl:id>
        <rdfs:label>T&apos;aet&apos;an County</rdfs:label>
    </owl:NamedIndividual>
    


    <!-- http://purl.obolibrary.org/obo/GAZ_00027762 -->

    <owl:NamedIndividual rdf:about="http://purl.obolibrary.org/obo/GAZ_00027762">
        <obo:RO_0001025 rdf:resource="http://purl.obolibrary.org/obo/GAZ_02000758"/>
        <obo:IAO_0000115>A county in Kangwon Province, North Korea. It was formed in 1952 from portions of Hoeyang, Yanggu, and Inje, in 1952.</obo:IAO_0000115>
        <oboInOwl:hasOBONamespace>GAZ</oboInOwl:hasOBONamespace>
        <oboInOwl:id>GAZ:00027762</oboInOwl:id>
        <rdfs:label>Kumgang County</rdfs:label>
    </owl:NamedIndividual>
    


    <!-- http://purl.obolibrary.org/obo/GAZ_00027763 -->

    <owl:NamedIndividual rdf:about="http://purl.obolibrary.org/obo/GAZ_00027763">
        <obo:RO_0001025 rdf:resource="http://purl.obolibrary.org/obo/GAZ_02000758"/>
        <obo:IAO_0000115>A county in Kangwon Province, North Korea. Originally part of Munchon, it was made a separate county in 1952-12.</obo:IAO_0000115>
        <oboInOwl:hasOBONamespace>GAZ</oboInOwl:hasOBONamespace>
        <oboInOwl:id>GAZ:00027763</oboInOwl:id>
        <rdfs:label>Ch&apos;onnae County</rdfs:label>
    </owl:NamedIndividual>
    


    <!-- http://purl.obolibrary.org/obo/GAZ_00027764 -->

    <owl:NamedIndividual rdf:about="http://purl.obolibrary.org/obo/GAZ_00027764">
        <obo:RO_0001025 rdf:resource="http://purl.obolibrary.org/obo/GAZ_02000758"/>
        <obo:IAO_0000115>A county in Kangwon Province, North Korea. Originally part of Kimhwa, it was split off as a separate county in 1952. Changdo lies to the west of the Taebaek Mountains, in the Ryongso region of Kangwon.</obo:IAO_0000115>
        <oboInOwl:hasOBONamespace>GAZ</oboInOwl:hasOBONamespace>
        <oboInOwl:id>GAZ:00027764</oboInOwl:id>
        <rdfs:label>Ch&apos;angdo County</rdfs:label>
    </owl:NamedIndividual>
    


    <!-- http://purl.obolibrary.org/obo/GAZ_00027765 -->

    <owl:NamedIndividual rdf:about="http://purl.obolibrary.org/obo/GAZ_00027765">
        <obo:RO_0001025 rdf:resource="http://purl.obolibrary.org/obo/GAZ_02000764"/>
        <obo:IAO_0000115>A populated place. A city in North Hwanghae Province, southern North Korea (DPRK), a former Directly Governed City.</obo:IAO_0000115>
        <oboInOwl:hasOBONamespace>GAZ</oboInOwl:hasOBONamespace>
        <oboInOwl:id>GAZ:00027765</oboInOwl:id>
        <rdfs:label>Kaesong City</rdfs:label>
    </owl:NamedIndividual>
    


    <!-- http://purl.obolibrary.org/obo/GAZ_00027766 -->

    <owl:NamedIndividual rdf:about="http://purl.obolibrary.org/obo/GAZ_00027766">
        <obo:RO_0001025 rdf:resource="http://purl.obolibrary.org/obo/GAZ_02000761"/>
        <obo:IAO_0000115>A county of Hwanghae-nam Province, North Korea.</obo:IAO_0000115>
        <oboInOwl:hasOBONamespace>GAZ</oboInOwl:hasOBONamespace>
        <oboInOwl:id>GAZ:00027766</oboInOwl:id>
        <rdfs:label>Pyoksong County</rdfs:label>
    </owl:NamedIndividual>
    


    <!-- http://purl.obolibrary.org/obo/GAZ_00027767 -->

    <owl:NamedIndividual rdf:about="http://purl.obolibrary.org/obo/GAZ_00027767">
        <obo:RO_0001025 rdf:resource="http://purl.obolibrary.org/obo/GAZ_02000764"/>
        <obo:IAO_0000115>A county of Hwanghae-buk Province.</obo:IAO_0000115>
        <oboInOwl:hasOBONamespace>GAZ</oboInOwl:hasOBONamespace>
        <oboInOwl:id>GAZ:00027767</oboInOwl:id>
        <rdfs:label>Changp&apos;ung County</rdfs:label>
    </owl:NamedIndividual>
    


    <!-- http://purl.obolibrary.org/obo/GAZ_00027768 -->

    <owl:NamedIndividual rdf:about="http://purl.obolibrary.org/obo/GAZ_00027768">
        <obo:RO_0001025 rdf:resource="http://purl.obolibrary.org/obo/GAZ_02000764"/>
        <obo:IAO_0000115>A city on the Taedong River in North Hwanghae Province, North Korea.</obo:IAO_0000115>
        <oboInOwl:hasOBONamespace>GAZ</oboInOwl:hasOBONamespace>
        <oboInOwl:id>GAZ:00027768</oboInOwl:id>
        <rdfs:label>Songrim City</rdfs:label>
    </owl:NamedIndividual>
    


    <!-- http://purl.obolibrary.org/obo/GAZ_00027769 -->

    <owl:NamedIndividual rdf:about="http://purl.obolibrary.org/obo/GAZ_00027769">
        <obo:RO_0001025 rdf:resource="http://purl.obolibrary.org/obo/GAZ_02000761"/>
        <obo:IAO_0000115>A county of Hwanghae-nam Province, North Korea.</obo:IAO_0000115>
        <oboInOwl:hasOBONamespace>GAZ</oboInOwl:hasOBONamespace>
        <oboInOwl:id>GAZ:00027769</oboInOwl:id>
        <rdfs:label>Sinch&apos;on County</rdfs:label>
    </owl:NamedIndividual>
    


    <!-- http://purl.obolibrary.org/obo/GAZ_00027770 -->

    <owl:NamedIndividual rdf:about="http://purl.obolibrary.org/obo/GAZ_00027770">
        <obo:RO_0001025 rdf:resource="http://purl.obolibrary.org/obo/GAZ_02000766"/>
        <obo:IAO_0000115>A special district of South Hamgyong province, near the city of Sinpo. Kumho was part of Sinpo until 1995, when it was made a special area under the direct administration of the province.</obo:IAO_0000115>
        <oboInOwl:hasOBONamespace>GAZ</oboInOwl:hasOBONamespace>
        <oboInOwl:id>GAZ:00027770</oboInOwl:id>
        <rdfs:label>Kumho Special District</rdfs:label>
    </owl:NamedIndividual>
    


    <!-- http://purl.obolibrary.org/obo/GAZ_00027771 -->

    <owl:NamedIndividual rdf:about="http://purl.obolibrary.org/obo/GAZ_00027771">
        <obo:RO_0001025 rdf:resource="http://purl.obolibrary.org/obo/GAZ_02000761"/>
        <obo:IAO_0000115>A county of Hwanghae-nam Province, North Korea.</obo:IAO_0000115>
        <oboInOwl:hasOBONamespace>GAZ</oboInOwl:hasOBONamespace>
        <oboInOwl:id>GAZ:00027771</oboInOwl:id>
        <rdfs:label>Samch&apos;on County</rdfs:label>
    </owl:NamedIndividual>
    


    <!-- http://purl.obolibrary.org/obo/GAZ_00027772 -->

    <owl:NamedIndividual rdf:about="http://purl.obolibrary.org/obo/GAZ_00027772">
        <obo:RO_0001025 rdf:resource="http://purl.obolibrary.org/obo/GAZ_02000761"/>
        <obo:IAO_0000115>A county of Hwanghae-nam Province, North Korea.</obo:IAO_0000115>
        <oboInOwl:hasOBONamespace>GAZ</oboInOwl:hasOBONamespace>
        <oboInOwl:id>GAZ:00027772</oboInOwl:id>
        <rdfs:label>Changyon County</rdfs:label>
    </owl:NamedIndividual>
    


    <!-- http://purl.obolibrary.org/obo/GAZ_00027773 -->

    <owl:NamedIndividual rdf:about="http://purl.obolibrary.org/obo/GAZ_00027773">
        <obo:RO_0001025 rdf:resource="http://purl.obolibrary.org/obo/GAZ_02000761"/>
    </owl:NamedIndividual>
    


    <!-- http://purl.obolibrary.org/obo/GAZ_00027774 -->

    <owl:NamedIndividual rdf:about="http://purl.obolibrary.org/obo/GAZ_00027774">
        <obo:RO_0001025 rdf:resource="http://purl.obolibrary.org/obo/GAZ_02000761"/>
        <obo:IAO_0000115>A county of Hwanghae-nam Province, North Korea.</obo:IAO_0000115>
        <oboInOwl:hasOBONamespace>GAZ</oboInOwl:hasOBONamespace>
        <oboInOwl:id>GAZ:00027774</oboInOwl:id>
        <rdfs:label>Chaeryong County</rdfs:label>
    </owl:NamedIndividual>
    


    <!-- http://purl.obolibrary.org/obo/GAZ_00027775 -->

    <owl:NamedIndividual rdf:about="http://purl.obolibrary.org/obo/GAZ_00027775">
        <obo:RO_0001025 rdf:resource="http://purl.obolibrary.org/obo/GAZ_02000761"/>
        <obo:IAO_0000115>A county of Hwanghae-nam Province, North Korea.</obo:IAO_0000115>
        <oboInOwl:hasOBONamespace>GAZ</oboInOwl:hasOBONamespace>
        <oboInOwl:id>GAZ:00027775</oboInOwl:id>
        <rdfs:label>Pongch&apos;on County</rdfs:label>
    </owl:NamedIndividual>
    


    <!-- http://purl.obolibrary.org/obo/GAZ_00027776 -->

    <owl:NamedIndividual rdf:about="http://purl.obolibrary.org/obo/GAZ_00027776">
        <obo:RO_0001025 rdf:resource="http://purl.obolibrary.org/obo/GAZ_02000761"/>
        <obo:IAO_0000115>A county of Hwanghae-nam Province, North Korea.</obo:IAO_0000115>
        <oboInOwl:hasOBONamespace>GAZ</oboInOwl:hasOBONamespace>
        <oboInOwl:id>GAZ:00027776</oboInOwl:id>
        <rdfs:label>Paekch&apos;on County</rdfs:label>
    </owl:NamedIndividual>
    


    <!-- http://purl.obolibrary.org/obo/GAZ_00027777 -->

    <owl:NamedIndividual rdf:about="http://purl.obolibrary.org/obo/GAZ_00027777">
        <obo:RO_0001025 rdf:resource="http://purl.obolibrary.org/obo/GAZ_02000764"/>
        <obo:IAO_0000115>A city; the capital of North Hwanghae Province, North Korea.</obo:IAO_0000115>
        <oboInOwl:hasOBONamespace>GAZ</oboInOwl:hasOBONamespace>
        <oboInOwl:id>GAZ:00027777</oboInOwl:id>
        <rdfs:label>Sariwon City</rdfs:label>
    </owl:NamedIndividual>
    


    <!-- http://purl.obolibrary.org/obo/GAZ_00027778 -->

    <owl:NamedIndividual rdf:about="http://purl.obolibrary.org/obo/GAZ_00027778">
        <obo:RO_0001025 rdf:resource="http://purl.obolibrary.org/obo/GAZ_02000764"/>
        <obo:IAO_0000115>A county of Hwanghae-buk Province.</obo:IAO_0000115>
        <oboInOwl:hasOBONamespace>GAZ</oboInOwl:hasOBONamespace>
        <oboInOwl:id>GAZ:00027778</oboInOwl:id>
        <rdfs:label>Kumch&apos;on County</rdfs:label>
    </owl:NamedIndividual>
    


    <!-- http://purl.obolibrary.org/obo/GAZ_00027779 -->

    <owl:NamedIndividual rdf:about="http://purl.obolibrary.org/obo/GAZ_00027779">
        <obo:RO_0001025 rdf:resource="http://purl.obolibrary.org/obo/GAZ_00128979"/>
        <obo:IAO_0000115>A county in southern Hwanghae-nam Province, North Korea. It is located on the Ongjin Peninsula, which projects into the Yellow Sea.</obo:IAO_0000115>
        <oboInOwl:hasOBONamespace>GAZ</oboInOwl:hasOBONamespace>
        <oboInOwl:id>GAZ:00027779</oboInOwl:id>
        <rdfs:label>Ongjin County</rdfs:label>
    </owl:NamedIndividual>
    


    <!-- http://purl.obolibrary.org/obo/GAZ_00027780 -->

    <owl:NamedIndividual rdf:about="http://purl.obolibrary.org/obo/GAZ_00027780">
        <obo:RO_0001025 rdf:resource="http://purl.obolibrary.org/obo/GAZ_02000761"/>
        <obo:IAO_0000115>A county of Hwanghae-nam Province, North Korea.</obo:IAO_0000115>
        <oboInOwl:hasOBONamespace>GAZ</oboInOwl:hasOBONamespace>
        <oboInOwl:id>GAZ:00027780</oboInOwl:id>
        <rdfs:label>Ch&apos;ongdan County</rdfs:label>
    </owl:NamedIndividual>
    


    <!-- http://purl.obolibrary.org/obo/GAZ_00027781 -->

    <owl:NamedIndividual rdf:about="http://purl.obolibrary.org/obo/GAZ_00027781">
        <obo:RO_0001025 rdf:resource="http://purl.obolibrary.org/obo/GAZ_02000761"/>
        <obo:IAO_0000115>A county of Hwanghae-nam Province, North Korea.</obo:IAO_0000115>
        <oboInOwl:hasOBONamespace>GAZ</oboInOwl:hasOBONamespace>
        <oboInOwl:id>GAZ:00027781</oboInOwl:id>
        <rdfs:label>Kangryong County</rdfs:label>
    </owl:NamedIndividual>
    


    <!-- http://purl.obolibrary.org/obo/GAZ_00027782 -->

    <owl:NamedIndividual rdf:about="http://purl.obolibrary.org/obo/GAZ_00027782">
        <obo:RO_0001025 rdf:resource="http://purl.obolibrary.org/obo/GAZ_02000761"/>
        <obo:IAO_0000115>A county in Hwanghae-nam Province, North Korea. It faces the Yellow Sea to the west.</obo:IAO_0000115>
        <oboInOwl:hasOBONamespace>GAZ</oboInOwl:hasOBONamespace>
        <oboInOwl:id>GAZ:00027782</oboInOwl:id>
        <rdfs:label>Kwail County</rdfs:label>
    </owl:NamedIndividual>
    


    <!-- http://purl.obolibrary.org/obo/GAZ_00027783 -->

    <owl:NamedIndividual rdf:about="http://purl.obolibrary.org/obo/GAZ_00027783">
        <obo:RO_0001025 rdf:resource="http://purl.obolibrary.org/obo/GAZ_02000761"/>
        <obo:IAO_0000115>A county of Hwanghae-nam Province, North Korea.</obo:IAO_0000115>
        <oboInOwl:hasOBONamespace>GAZ</oboInOwl:hasOBONamespace>
        <oboInOwl:id>GAZ:00027783</oboInOwl:id>
        <rdfs:label>Anak County</rdfs:label>
    </owl:NamedIndividual>
    


    <!-- http://purl.obolibrary.org/obo/GAZ_00027784 -->

    <owl:NamedIndividual rdf:about="http://purl.obolibrary.org/obo/GAZ_00027784">
        <obo:RO_0001025 rdf:resource="http://purl.obolibrary.org/obo/GAZ_02000766"/>
        <obo:IAO_0000115>A county in South Hamgyong province, North Korea. It was formed from part of Kowon County in 1990-12.</obo:IAO_0000115>
        <oboInOwl:hasOBONamespace>GAZ</oboInOwl:hasOBONamespace>
        <oboInOwl:id>GAZ:00027784</oboInOwl:id>
        <rdfs:label>Sudong County</rdfs:label>
    </owl:NamedIndividual>
    


    <!-- http://purl.obolibrary.org/obo/GAZ_00027785 -->

    <owl:NamedIndividual rdf:about="http://purl.obolibrary.org/obo/GAZ_00027785">
        <obo:RO_0001025 rdf:resource="http://purl.obolibrary.org/obo/GAZ_02000764"/>
        <obo:IAO_0000115>A county of Hwanghae-buk Province.</obo:IAO_0000115>
        <oboInOwl:hasOBONamespace>GAZ</oboInOwl:hasOBONamespace>
        <oboInOwl:id>GAZ:00027785</oboInOwl:id>
        <rdfs:label>Koksan County</rdfs:label>
    </owl:NamedIndividual>
    


    <!-- http://purl.obolibrary.org/obo/GAZ_00027786 -->

    <owl:NamedIndividual rdf:about="http://purl.obolibrary.org/obo/GAZ_00027786">
        <obo:RO_0001025 rdf:resource="http://purl.obolibrary.org/obo/GAZ_02000764"/>
        <obo:IAO_0000115>A county of Hwanghae-buk Province.</obo:IAO_0000115>
        <oboInOwl:hasOBONamespace>GAZ</oboInOwl:hasOBONamespace>
        <oboInOwl:id>GAZ:00027786</oboInOwl:id>
        <rdfs:label>P&apos;yongsan County</rdfs:label>
    </owl:NamedIndividual>
    


    <!-- http://purl.obolibrary.org/obo/GAZ_00027787 -->

    <owl:NamedIndividual rdf:about="http://purl.obolibrary.org/obo/GAZ_00027787">
        <obo:RO_0001025 rdf:resource="http://purl.obolibrary.org/obo/GAZ_02000764"/>
        <obo:IAO_0000115>A county of Hwanghae-buk Province.</obo:IAO_0000115>
        <oboInOwl:hasOBONamespace>GAZ</oboInOwl:hasOBONamespace>
        <oboInOwl:id>GAZ:00027787</oboInOwl:id>
        <rdfs:label>Sinp&apos;yong County</rdfs:label>
    </owl:NamedIndividual>
    


    <!-- http://purl.obolibrary.org/obo/GAZ_00027788 -->

    <owl:NamedIndividual rdf:about="http://purl.obolibrary.org/obo/GAZ_00027788">
        <obo:RO_0001025 rdf:resource="http://purl.obolibrary.org/obo/GAZ_02000764"/>
        <obo:IAO_0000115>A county of Hwanghae-buk Province.</obo:IAO_0000115>
        <oboInOwl:hasOBONamespace>GAZ</oboInOwl:hasOBONamespace>
        <oboInOwl:id>GAZ:00027788</oboInOwl:id>
        <rdfs:label>Hwangju County</rdfs:label>
    </owl:NamedIndividual>
    


    <!-- http://purl.obolibrary.org/obo/GAZ_00027789 -->

    <owl:NamedIndividual rdf:about="http://purl.obolibrary.org/obo/GAZ_00027789">
        <obo:RO_0001025 rdf:resource="http://purl.obolibrary.org/obo/GAZ_02000764"/>
        <obo:IAO_0000115>A county of Hwanghae-buk Province.</obo:IAO_0000115>
        <oboInOwl:hasOBONamespace>GAZ</oboInOwl:hasOBONamespace>
        <oboInOwl:id>GAZ:00027789</oboInOwl:id>
        <rdfs:label>Sin&apos;gye County</rdfs:label>
    </owl:NamedIndividual>
    


    <!-- http://purl.obolibrary.org/obo/GAZ_00027790 -->

    <owl:NamedIndividual rdf:about="http://purl.obolibrary.org/obo/GAZ_00027790">
        <obo:RO_0001025 rdf:resource="http://purl.obolibrary.org/obo/GAZ_02000764"/>
        <obo:IAO_0000115>A county of Hwanghae-buk Province.</obo:IAO_0000115>
        <oboInOwl:hasOBONamespace>GAZ</oboInOwl:hasOBONamespace>
        <oboInOwl:id>GAZ:00027790</oboInOwl:id>
        <rdfs:label>Pongsan County</rdfs:label>
    </owl:NamedIndividual>
    


    <!-- http://purl.obolibrary.org/obo/GAZ_00027791 -->

    <owl:NamedIndividual rdf:about="http://purl.obolibrary.org/obo/GAZ_00027791">
        <obo:RO_0001025 rdf:resource="http://purl.obolibrary.org/obo/GAZ_02000764"/>
        <obo:IAO_0000115>A county of Hwanghae-buk Province.</obo:IAO_0000115>
        <oboInOwl:hasOBONamespace>GAZ</oboInOwl:hasOBONamespace>
        <oboInOwl:id>GAZ:00027791</oboInOwl:id>
        <rdfs:label>Suan County</rdfs:label>
    </owl:NamedIndividual>
    


    <!-- http://purl.obolibrary.org/obo/GAZ_00027792 -->

    <owl:NamedIndividual rdf:about="http://purl.obolibrary.org/obo/GAZ_00027792">
        <obo:RO_0001025 rdf:resource="http://purl.obolibrary.org/obo/GAZ_02000764"/>
        <obo:IAO_0000115>A county of Hwanghae-buk Province.</obo:IAO_0000115>
        <oboInOwl:hasOBONamespace>GAZ</oboInOwl:hasOBONamespace>
        <oboInOwl:id>GAZ:00027792</oboInOwl:id>
        <rdfs:label>Rinsan County</rdfs:label>
    </owl:NamedIndividual>
    


    <!-- http://purl.obolibrary.org/obo/GAZ_00027793 -->

    <owl:NamedIndividual rdf:about="http://purl.obolibrary.org/obo/GAZ_00027793">
        <obo:RO_0001025 rdf:resource="http://purl.obolibrary.org/obo/GAZ_02000764"/>
        <obo:IAO_0000115>A county of Hwanghae-buk Province.</obo:IAO_0000115>
        <oboInOwl:hasOBONamespace>GAZ</oboInOwl:hasOBONamespace>
        <oboInOwl:id>GAZ:00027793</oboInOwl:id>
        <rdfs:label>Unp&apos;a County</rdfs:label>
    </owl:NamedIndividual>
    


    <!-- http://purl.obolibrary.org/obo/GAZ_00027794 -->

    <owl:NamedIndividual rdf:about="http://purl.obolibrary.org/obo/GAZ_00027794">
        <obo:RO_0001025 rdf:resource="http://purl.obolibrary.org/obo/GAZ_02000764"/>
        <obo:IAO_0000115>A county of Hwanghae-buk Province.</obo:IAO_0000115>
        <oboInOwl:hasOBONamespace>GAZ</oboInOwl:hasOBONamespace>
        <oboInOwl:id>GAZ:00027794</oboInOwl:id>
        <rdfs:label>Sohung County</rdfs:label>
    </owl:NamedIndividual>
    


    <!-- http://purl.obolibrary.org/obo/GAZ_00027795 -->

    <owl:NamedIndividual rdf:about="http://purl.obolibrary.org/obo/GAZ_00027795">
        <obo:RO_0001025 rdf:resource="http://purl.obolibrary.org/obo/GAZ_02000764"/>
        <obo:IAO_0000115>A county of Hwanghae-buk Province.</obo:IAO_0000115>
        <oboInOwl:hasOBONamespace>GAZ</oboInOwl:hasOBONamespace>
        <oboInOwl:id>GAZ:00027795</oboInOwl:id>
        <rdfs:label>Yontan County</rdfs:label>
    </owl:NamedIndividual>
    


    <!-- http://purl.obolibrary.org/obo/GAZ_00027796 -->

    <owl:NamedIndividual rdf:about="http://purl.obolibrary.org/obo/GAZ_00027796">
        <obo:RO_0001025 rdf:resource="http://purl.obolibrary.org/obo/GAZ_02000764"/>
        <obo:IAO_0000115>A county of Hwanghae-buk Province.</obo:IAO_0000115>
        <oboInOwl:hasOBONamespace>GAZ</oboInOwl:hasOBONamespace>
        <oboInOwl:id>GAZ:00027796</oboInOwl:id>
        <rdfs:label>Kaep&apos;ung County</rdfs:label>
    </owl:NamedIndividual>
    


    <!-- http://purl.obolibrary.org/obo/GAZ_00027797 -->

    <owl:NamedIndividual rdf:about="http://purl.obolibrary.org/obo/GAZ_00027797">
        <obo:RO_0001025 rdf:resource="http://purl.obolibrary.org/obo/GAZ_02000766"/>
        <obo:IAO_0000115>A port city on the coast of the Sea of Japan (East Sea of Korea) in central South Hamgyong province, North Korea.</obo:IAO_0000115>
        <oboInOwl:hasOBONamespace>GAZ</oboInOwl:hasOBONamespace>
        <oboInOwl:id>GAZ:00027797</oboInOwl:id>
        <rdfs:label>Sinp&apos;o City</rdfs:label>
    </owl:NamedIndividual>
    


    <!-- http://purl.obolibrary.org/obo/GAZ_00027798 -->

    <owl:NamedIndividual rdf:about="http://purl.obolibrary.org/obo/GAZ_00027798">
        <obo:RO_0001025 rdf:resource="http://purl.obolibrary.org/obo/GAZ_02000764"/>
        <obo:IAO_0000115>A county of Hwanghae-buk Province.</obo:IAO_0000115>
        <oboInOwl:hasOBONamespace>GAZ</oboInOwl:hasOBONamespace>
        <oboInOwl:id>GAZ:00027798</oboInOwl:id>
        <rdfs:label>T&apos;osan County</rdfs:label>
    </owl:NamedIndividual>
    


    <!-- http://purl.obolibrary.org/obo/GAZ_00027799 -->

    <owl:NamedIndividual rdf:about="http://purl.obolibrary.org/obo/GAZ_00027799">
        <obo:RO_0001025 rdf:resource="http://purl.obolibrary.org/obo/GAZ_02000766"/>
        <obo:IAO_0000115>A populated place. A city in North Korea; the capital of South Hamgyong Province. Hamhung is on the left branch of the Songch&apos;on River, on the eastern part of the Hamhung plain, in Hamgyong-buk Province, northeast North Korea.</obo:IAO_0000115>
        <oboInOwl:hasOBONamespace>GAZ</oboInOwl:hasOBONamespace>
        <oboInOwl:id>GAZ:00027799</oboInOwl:id>
        <rdfs:label>Hamhung City</rdfs:label>
    </owl:NamedIndividual>
    


    <!-- http://purl.obolibrary.org/obo/GAZ_00027800 -->

    <owl:NamedIndividual rdf:about="http://purl.obolibrary.org/obo/GAZ_00027800">
        <obo:RO_0001025 rdf:resource="http://purl.obolibrary.org/obo/GAZ_02000766"/>
        <obo:IAO_0000115>A populated place. A city in northeastern South Hamgyong province, North Korea. Tanchon borders the Sea of Japan (East Sea of Korea), into which the Namdae River flows.</obo:IAO_0000115>
        <oboInOwl:hasOBONamespace>GAZ</oboInOwl:hasOBONamespace>
        <oboInOwl:id>GAZ:00027800</oboInOwl:id>
        <rdfs:label>Tanch&apos;on City</rdfs:label>
    </owl:NamedIndividual>
    


    <!-- http://purl.obolibrary.org/obo/GAZ_00027801 -->

    <owl:NamedIndividual rdf:about="http://purl.obolibrary.org/obo/GAZ_00027801">
        <obo:RO_0001025 rdf:resource="http://purl.obolibrary.org/obo/GAZ_00027799"/>
        <obo:IAO_0000115>A former port city on the eastern coast of South Hamgyong Province, North Korea, on the Sea of Japan. In late 2005, Hungnam was demoted from Hungnam-si to Hungnam-kuyok (Hungnam District) within Hamhung-si.</obo:IAO_0000115>
        <oboInOwl:hasOBONamespace>GAZ</oboInOwl:hasOBONamespace>
        <oboInOwl:id>GAZ:00027801</oboInOwl:id>
        <rdfs:label>Hungnam District</rdfs:label>
    </owl:NamedIndividual>
    


    <!-- http://purl.obolibrary.org/obo/GAZ_00027802 -->

    <owl:NamedIndividual rdf:about="http://purl.obolibrary.org/obo/GAZ_00027802">
        <obo:RO_0001025 rdf:resource="http://purl.obolibrary.org/obo/GAZ_02000766"/>
        <obo:IAO_0000115>A county in South Hamgyong province, North Korea. It borders the Sea of Japan (East Sea of Korea) to the south and east.</obo:IAO_0000115>
        <oboInOwl:hasOBONamespace>GAZ</oboInOwl:hasOBONamespace>
        <oboInOwl:id>GAZ:00027802</oboInOwl:id>
        <rdfs:label>Ragwon County</rdfs:label>
    </owl:NamedIndividual>
    


    <!-- http://purl.obolibrary.org/obo/GAZ_00027803 -->

    <owl:NamedIndividual rdf:about="http://purl.obolibrary.org/obo/GAZ_00027803">
        <obo:RO_0001025 rdf:resource="http://purl.obolibrary.org/obo/GAZ_02000766"/>
        <obo:IAO_0000115>A county in South Hamgyong province, North Korea.</obo:IAO_0000115>
        <oboInOwl:hasOBONamespace>GAZ</oboInOwl:hasOBONamespace>
        <oboInOwl:id>GAZ:00027803</oboInOwl:id>
        <rdfs:label>Toksong County</rdfs:label>
    </owl:NamedIndividual>
    


    <!-- http://purl.obolibrary.org/obo/GAZ_00027804 -->

    <owl:NamedIndividual rdf:about="http://purl.obolibrary.org/obo/GAZ_00027804">
        <obo:RO_0001025 rdf:resource="http://purl.obolibrary.org/obo/GAZ_02000766"/>
        <obo:IAO_0000115>A mountainous county in South Hamgyong province, North Korea. It is traversed by the Hamgyong and Palbong ranges.</obo:IAO_0000115>
        <oboInOwl:hasOBONamespace>GAZ</oboInOwl:hasOBONamespace>
        <oboInOwl:id>GAZ:00027804</oboInOwl:id>
        <rdfs:label>Sinhung County</rdfs:label>
    </owl:NamedIndividual>
    


    <!-- http://purl.obolibrary.org/obo/GAZ_00027805 -->

    <owl:NamedIndividual rdf:about="http://purl.obolibrary.org/obo/GAZ_00027805">
        <obo:RO_0001025 rdf:resource="http://purl.obolibrary.org/obo/GAZ_02000766"/>
        <obo:IAO_0000115>A county in South Hamgyong province, North Korea. It lies at the southern tip of the province.</obo:IAO_0000115>
        <oboInOwl:hasOBONamespace>GAZ</oboInOwl:hasOBONamespace>
        <oboInOwl:id>GAZ:00027805</oboInOwl:id>
        <rdfs:label>Kowon County</rdfs:label>
    </owl:NamedIndividual>
    


    <!-- http://purl.obolibrary.org/obo/GAZ_00027806 -->

    <owl:NamedIndividual rdf:about="http://purl.obolibrary.org/obo/GAZ_00027806">
        <obo:RO_0001025 rdf:resource="http://purl.obolibrary.org/obo/GAZ_02000766"/>
        <obo:IAO_0000115>A county in South Hamgyong province, North Korea. Originally part of Yonghung County, it became a separate entity as part of the 1952.</obo:IAO_0000115>
        <oboInOwl:hasOBONamespace>GAZ</oboInOwl:hasOBONamespace>
        <oboInOwl:id>GAZ:00027806</oboInOwl:id>
        <rdfs:label>Yodok County</rdfs:label>
    </owl:NamedIndividual>
    


    <!-- http://purl.obolibrary.org/obo/GAZ_00027807 -->

    <owl:NamedIndividual rdf:about="http://purl.obolibrary.org/obo/GAZ_00027807">
        <obo:RO_0001025 rdf:resource="http://purl.obolibrary.org/obo/GAZ_02000766"/>
        <obo:IAO_0000115>A county in South Hamgyong province, North Korea. It borders South Pyongan province to the south, and the East Korea Bay to the east.</obo:IAO_0000115>
        <oboInOwl:hasOBONamespace>GAZ</oboInOwl:hasOBONamespace>
        <oboInOwl:id>GAZ:00027807</oboInOwl:id>
        <rdfs:label>Ch&apos;ongp&apos;yong County</rdfs:label>
    </owl:NamedIndividual>
    


    <!-- http://purl.obolibrary.org/obo/GAZ_00027808 -->

    <owl:NamedIndividual rdf:about="http://purl.obolibrary.org/obo/GAZ_00027808">
        <obo:RO_0001025 rdf:resource="http://purl.obolibrary.org/obo/GAZ_02000766"/>
        <obo:IAO_0000115>A county in South Hamgyong province, North Korea. It was created after the division of Korea, from portions of Tanchon and Pungsan.</obo:IAO_0000115>
        <oboInOwl:hasOBONamespace>GAZ</oboInOwl:hasOBONamespace>
        <oboInOwl:id>GAZ:00027808</oboInOwl:id>
        <rdfs:label>Hoch&apos;on County</rdfs:label>
    </owl:NamedIndividual>
    


    <!-- http://purl.obolibrary.org/obo/GAZ_00027809 -->

    <owl:NamedIndividual rdf:about="http://purl.obolibrary.org/obo/GAZ_00027809">
        <obo:RO_0001025 rdf:resource="http://purl.obolibrary.org/obo/GAZ_02000766"/>
        <obo:IAO_0000115>A county in South Hamgyong province, North Korea. It was originally part of Hamju County, from which it was separated in 1952.</obo:IAO_0000115>
        <oboInOwl:hasOBONamespace>GAZ</oboInOwl:hasOBONamespace>
        <oboInOwl:id>GAZ:00027809</oboInOwl:id>
        <rdfs:label>Yonggwang County</rdfs:label>
    </owl:NamedIndividual>
    


    <!-- http://purl.obolibrary.org/obo/GAZ_00027810 -->

    <owl:NamedIndividual rdf:about="http://purl.obolibrary.org/obo/GAZ_00027810">
        <obo:RO_0001025 rdf:resource="http://purl.obolibrary.org/obo/GAZ_02000766"/>
        <obo:IAO_0000115>A county in South Hamgyong province, North Korea. It is flanked by the Sea of Japan (East Sea of Korea) to the south, and by the Hamgyong Mountains to the north.</obo:IAO_0000115>
        <oboInOwl:hasOBONamespace>GAZ</oboInOwl:hasOBONamespace>
        <oboInOwl:id>GAZ:00027810</oboInOwl:id>
        <rdfs:label>Hongwon County</rdfs:label>
    </owl:NamedIndividual>
    


    <!-- http://purl.obolibrary.org/obo/GAZ_00027811 -->

    <owl:NamedIndividual rdf:about="http://purl.obolibrary.org/obo/GAZ_00027811">
        <obo:RO_0001025 rdf:resource="http://purl.obolibrary.org/obo/GAZ_02000766"/>
        <obo:IAO_0000115>A county in South Hamgyong province, North Korea. It borders the Sea of Japan (East Sea of Korea) to the east.</obo:IAO_0000115>
        <oboInOwl:hasOBONamespace>GAZ</oboInOwl:hasOBONamespace>
        <oboInOwl:id>GAZ:00027811</oboInOwl:id>
        <rdfs:label>Kumya County</rdfs:label>
    </owl:NamedIndividual>
    


    <!-- http://purl.obolibrary.org/obo/GAZ_00027812 -->

    <owl:NamedIndividual rdf:about="http://purl.obolibrary.org/obo/GAZ_00027812">
        <obo:RO_0001025 rdf:resource="http://purl.obolibrary.org/obo/GAZ_02000766"/>
        <obo:IAO_0000115>A county in eastern South Hamgyong province, North Korea. It borders the Sea of Japan (East Sea of Korea) to the south.</obo:IAO_0000115>
        <oboInOwl:hasOBONamespace>GAZ</oboInOwl:hasOBONamespace>
        <oboInOwl:id>GAZ:00027812</oboInOwl:id>
        <rdfs:label>Pukch&apos;ong County</rdfs:label>
    </owl:NamedIndividual>
    


    <!-- http://purl.obolibrary.org/obo/GAZ_00027813 -->

    <owl:NamedIndividual rdf:about="http://purl.obolibrary.org/obo/GAZ_00027813">
        <obo:RO_0001025 rdf:resource="http://purl.obolibrary.org/obo/GAZ_02000766"/>
        <obo:IAO_0000115>A mountainous county in South Hamgyong province, North Korea.</obo:IAO_0000115>
        <oboInOwl:hasOBONamespace>GAZ</oboInOwl:hasOBONamespace>
        <oboInOwl:id>GAZ:00027813</oboInOwl:id>
        <rdfs:label>Changjin County</rdfs:label>
    </owl:NamedIndividual>
    


    <!-- http://purl.obolibrary.org/obo/GAZ_00027814 -->

    <owl:NamedIndividual rdf:about="http://purl.obolibrary.org/obo/GAZ_00027814">
        <obo:RO_0001025 rdf:resource="http://purl.obolibrary.org/obo/GAZ_02000766"/>
        <obo:IAO_0000115>A county in northern South Hamgyong province, North Korea.</obo:IAO_0000115>
        <oboInOwl:hasOBONamespace>GAZ</oboInOwl:hasOBONamespace>
        <oboInOwl:id>GAZ:00027814</oboInOwl:id>
        <rdfs:label>Pujon County</rdfs:label>
    </owl:NamedIndividual>
    


    <!-- http://purl.obolibrary.org/obo/GAZ_00027815 -->

    <owl:NamedIndividual rdf:about="http://purl.obolibrary.org/obo/GAZ_00027815">
        <obo:RO_0001025 rdf:resource="http://purl.obolibrary.org/obo/GAZ_02000766"/>
        <obo:IAO_0000115>A county in South Hamgyong province, North Korea.</obo:IAO_0000115>
        <oboInOwl:hasOBONamespace>GAZ</oboInOwl:hasOBONamespace>
        <oboInOwl:id>GAZ:00027815</oboInOwl:id>
        <rdfs:label>Hamju County</rdfs:label>
    </owl:NamedIndividual>
    


    <!-- http://purl.obolibrary.org/obo/GAZ_00027816 -->

    <owl:NamedIndividual rdf:about="http://purl.obolibrary.org/obo/GAZ_00027816">
        <obo:RO_0001025 rdf:resource="http://purl.obolibrary.org/obo/GAZ_02000766"/>
        <obo:IAO_0000115>A county in South Hamgyong province, North Korea. It is located at the province&apos;s northeastern tip, and borders the Sea of Japan (East Sea of Korea) to the southeast.</obo:IAO_0000115>
        <oboInOwl:hasOBONamespace>GAZ</oboInOwl:hasOBONamespace>
        <oboInOwl:id>GAZ:00027816</oboInOwl:id>
        <rdfs:label>Riwon County</rdfs:label>
    </owl:NamedIndividual>
    


    <!-- http://purl.obolibrary.org/obo/GAZ_00027817 -->

    <owl:NamedIndividual rdf:about="http://purl.obolibrary.org/obo/GAZ_00027817">
        <obo:RO_0001025 rdf:resource="http://purl.obolibrary.org/obo/GAZ_02000763"/>
        <obo:IAO_0000115>A county in North Hamgyong province, North Korea. It is situated on the coast of the Sea of Japan. Originally part of Kyongsong county, Orang was created in 1952.</obo:IAO_0000115>
        <oboInOwl:hasOBONamespace>GAZ</oboInOwl:hasOBONamespace>
        <oboInOwl:id>GAZ:00027817</oboInOwl:id>
        <rdfs:label>Orang County</rdfs:label>
    </owl:NamedIndividual>
    


    <!-- http://purl.obolibrary.org/obo/GAZ_00027818 -->

    <owl:NamedIndividual rdf:about="http://purl.obolibrary.org/obo/GAZ_00027818">
        <obo:RO_0001025 rdf:resource="http://purl.obolibrary.org/obo/GAZ_02000763"/>
        <obo:IAO_0000115>A county in North Hamgyong province, North Korea.</obo:IAO_0000115>
        <oboInOwl:hasOBONamespace>GAZ</oboInOwl:hasOBONamespace>
        <oboInOwl:id>GAZ:00027818</oboInOwl:id>
        <rdfs:label>Myongch&apos;on County</rdfs:label>
    </owl:NamedIndividual>
    


    <!-- http://purl.obolibrary.org/obo/GAZ_00027819 -->

    <owl:NamedIndividual rdf:about="http://purl.obolibrary.org/obo/GAZ_00027819">
        <obo:RO_0001025 rdf:resource="http://purl.obolibrary.org/obo/GAZ_02000763"/>
        <obo:IAO_0000115>A county in North Hamgyong province, North Korea. The county borders the People&apos;s Republic of China to the northeast.</obo:IAO_0000115>
        <oboInOwl:hasOBONamespace>GAZ</oboInOwl:hasOBONamespace>
        <oboInOwl:id>GAZ:00027819</oboInOwl:id>
        <rdfs:label>Undok County</rdfs:label>
    </owl:NamedIndividual>
    


    <!-- http://purl.obolibrary.org/obo/GAZ_00027820 -->

    <owl:NamedIndividual rdf:about="http://purl.obolibrary.org/obo/GAZ_00027820">
        <obo:RO_0001025 rdf:resource="http://purl.obolibrary.org/obo/GAZ_02000763"/>
        <obo:IAO_0000115>A county in North Hamgyong province, North Korea.</obo:IAO_0000115>
        <oboInOwl:hasOBONamespace>GAZ</oboInOwl:hasOBONamespace>
        <oboInOwl:id>GAZ:00027820</oboInOwl:id>
        <rdfs:label>Puryong County</rdfs:label>
    </owl:NamedIndividual>
    


    <!-- http://purl.obolibrary.org/obo/GAZ_00027821 -->

    <owl:NamedIndividual rdf:about="http://purl.obolibrary.org/obo/GAZ_00027821">
        <obo:RO_0001025 rdf:resource="http://purl.obolibrary.org/obo/GAZ_02000763"/>
        <obo:IAO_0000115>A county in North Hamgyong province, North Korea. The county seat is Kilchu-up. It is located in the southern part of North Hamgyong. It borders Myongch&apos;on on the east, Kimch&apos;aek and Hwadae to the south, Hwasong and Orang to the north. To the west it borders Tanch&apos;on in South Hamgyong and Paegam in Ryanggang.</obo:IAO_0000115>
        <oboInOwl:hasOBONamespace>GAZ</oboInOwl:hasOBONamespace>
        <oboInOwl:id>GAZ:00027821</oboInOwl:id>
        <rdfs:label>Kilchu County</rdfs:label>
    </owl:NamedIndividual>
    


    <!-- http://purl.obolibrary.org/obo/GAZ_00027822 -->

    <owl:NamedIndividual rdf:about="http://purl.obolibrary.org/obo/GAZ_00027822">
        <obo:RO_0001025 rdf:resource="http://purl.obolibrary.org/obo/GAZ_02000763"/>
        <obo:IAO_0000115>A county on the central coast of North Hamgyong, North Korea.</obo:IAO_0000115>
        <oboInOwl:hasOBONamespace>GAZ</oboInOwl:hasOBONamespace>
        <oboInOwl:id>GAZ:00027822</oboInOwl:id>
        <rdfs:label>Kyongsong County</rdfs:label>
    </owl:NamedIndividual>
    


    <!-- http://purl.obolibrary.org/obo/GAZ_00027823 -->

    <owl:NamedIndividual rdf:about="http://purl.obolibrary.org/obo/GAZ_00027823">
        <obo:RO_0001025 rdf:resource="http://purl.obolibrary.org/obo/GAZ_02000763"/>
        <obo:IAO_0000115>A county in central North Hamgyong province, North Korea. It borders the People&apos;s Republic of China to the north, across the Tumen River.</obo:IAO_0000115>
        <oboInOwl:hasOBONamespace>GAZ</oboInOwl:hasOBONamespace>
        <oboInOwl:id>GAZ:00027823</oboInOwl:id>
        <rdfs:label>Musan County</rdfs:label>
    </owl:NamedIndividual>
    


    <!-- http://purl.obolibrary.org/obo/GAZ_00027824 -->

    <owl:NamedIndividual rdf:about="http://purl.obolibrary.org/obo/GAZ_00027824">
        <obo:RO_0001025 rdf:resource="http://purl.obolibrary.org/obo/GAZ_02000763"/>
        <obo:IAO_0000115>A county in southern North Hamgyong province, North Korea. It adjoins the Sea of Japan on the east and south. By land, it adjoins Kimchaek and Kilchu to the west, and Myongch&apos;on to the north. The county was formed from parts of Kilchu and Myongch&apos;on in the 1950s.</obo:IAO_0000115>
        <oboInOwl:hasOBONamespace>GAZ</oboInOwl:hasOBONamespace>
        <oboInOwl:id>GAZ:00027824</oboInOwl:id>
        <rdfs:label>Hwadae County</rdfs:label>
    </owl:NamedIndividual>
    


    <!-- http://purl.obolibrary.org/obo/GAZ_00027825 -->

    <owl:NamedIndividual rdf:about="http://purl.obolibrary.org/obo/GAZ_00027825">
        <obo:RO_0001025 rdf:resource="http://purl.obolibrary.org/obo/GAZ_02000763"/>
        <obo:IAO_0000115>A county in North Hamgyong province, North Korea. Hwasong abuts the Sea of Japan.</obo:IAO_0000115>
        <oboInOwl:hasOBONamespace>GAZ</oboInOwl:hasOBONamespace>
        <oboInOwl:id>GAZ:00027825</oboInOwl:id>
        <rdfs:label>Hwasong County</rdfs:label>
    </owl:NamedIndividual>
    


    <!-- http://purl.obolibrary.org/obo/GAZ_00027826 -->

    <owl:NamedIndividual rdf:about="http://purl.obolibrary.org/obo/GAZ_00027826">
        <obo:RO_0001025 rdf:resource="http://purl.obolibrary.org/obo/GAZ_02000763"/>
        <obo:IAO_0000115>A populated place. A city in North Korea. It is the capital of the North Hamgyong Province in North Korea. From 1960 to 1967 and again from 1977 to 1985, Ch&apos;ongjin was administered separately from NHamgyong-buk Province as a Directly Governed City (Chikhalsi). Prior to 1960, from 1967 to 1977, and since 1985, the city has been part of the North Hamgyong Province.</obo:IAO_0000115>
        <oboInOwl:hasOBONamespace>GAZ</oboInOwl:hasOBONamespace>
        <oboInOwl:id>GAZ:00027826</oboInOwl:id>
        <rdfs:label>Ch&apos;ongjin City</rdfs:label>
    </owl:NamedIndividual>
    


    <!-- http://purl.obolibrary.org/obo/GAZ_00027827 -->

    <owl:NamedIndividual rdf:about="http://purl.obolibrary.org/obo/GAZ_00027827">
        <obo:RO_0001025 rdf:resource="http://purl.obolibrary.org/obo/GAZ_02000763"/>
        <obo:IAO_0000115>A populated place. A city in North Hamgyong Province, North Korea.</obo:IAO_0000115>
        <oboInOwl:hasOBONamespace>GAZ</oboInOwl:hasOBONamespace>
        <oboInOwl:id>GAZ:00027827</oboInOwl:id>
        <rdfs:label>Kimch&apos;aek City</rdfs:label>
    </owl:NamedIndividual>
    


    <!-- http://purl.obolibrary.org/obo/GAZ_00027828 -->

    <owl:NamedIndividual rdf:about="http://purl.obolibrary.org/obo/GAZ_00027828">
        <obo:RO_0001025 rdf:resource="http://purl.obolibrary.org/obo/GAZ_02000763"/>
        <obo:IAO_0000115>A county in North Hamgyong province, North Korea. It borders the People&apos;s Republic of China to the east.</obo:IAO_0000115>
        <oboInOwl:hasOBONamespace>GAZ</oboInOwl:hasOBONamespace>
        <oboInOwl:id>GAZ:00027828</oboInOwl:id>
        <rdfs:label>Saebyol County</rdfs:label>
    </owl:NamedIndividual>
    


    <!-- http://purl.obolibrary.org/obo/GAZ_00027829 -->

    <owl:NamedIndividual rdf:about="http://purl.obolibrary.org/obo/GAZ_00027829">
        <obo:RO_0001025 rdf:resource="http://purl.obolibrary.org/obo/GAZ_02000763"/>
        <obo:IAO_0000115>A county in North Hamgyong Province, North Korea,located near the border with China.</obo:IAO_0000115>
        <oboInOwl:hasOBONamespace>GAZ</oboInOwl:hasOBONamespace>
        <oboInOwl:id>GAZ:00027829</oboInOwl:id>
        <rdfs:label>Onsong County</rdfs:label>
    </owl:NamedIndividual>
    


    <!-- http://purl.obolibrary.org/obo/GAZ_00027830 -->

    <owl:NamedIndividual rdf:about="http://purl.obolibrary.org/obo/GAZ_00027830">
        <obo:RO_0001025 rdf:resource="http://purl.obolibrary.org/obo/GAZ_02000763"/>
        <obo:IAO_0000115>A populated place. A city in North Hamgyong Province, North Korea. It is opposite Jilin Province, China, with the Tumen River in between.</obo:IAO_0000115>
        <oboInOwl:hasOBONamespace>GAZ</oboInOwl:hasOBONamespace>
        <oboInOwl:id>GAZ:00027830</oboInOwl:id>
        <rdfs:label>Hoeryong City</rdfs:label>
    </owl:NamedIndividual>
    


    <!-- http://purl.obolibrary.org/obo/GAZ_00027831 -->

    <owl:NamedIndividual rdf:about="http://purl.obolibrary.org/obo/GAZ_00027831">
        <obo:RO_0001025 rdf:resource="http://purl.obolibrary.org/obo/GAZ_02000763"/>
        <obo:IAO_0000115>A county in North Hamgyong province, North Korea. It was created following the division of Korea, being split off from Musan county in the 1952 reorganization of local government.</obo:IAO_0000115>
        <oboInOwl:hasOBONamespace>GAZ</oboInOwl:hasOBONamespace>
        <oboInOwl:id>GAZ:00027831</oboInOwl:id>
        <rdfs:label>Yonsa County</rdfs:label>
    </owl:NamedIndividual>
    


    <!-- http://purl.obolibrary.org/obo/GAZ_00052993 -->

    <owl:NamedIndividual rdf:about="http://purl.obolibrary.org/obo/GAZ_00052993">
        <obo:RO_0001025 rdf:resource="http://purl.obolibrary.org/obo/GAZ_00054834"/>
        <obo:IAO_0000115>A volcanic mountain on the border between China and North Korea. A massive stratovolcano is a relatively unknown, but volcanologically significant volcano straddling the China/Korea border. A 5 km wide, 850-m-deep summit caldera is filled by scenic Lake Tianchi (Sky Lake). A large Korean-speaking population resides near the volcano on both sides of the border. The 60 km-diameter dominantly trachytic and rhyolitic volcano was constructed over the Changbaishan (Laoheidingzi) shield volcano. Satellitic cinder cones are aligned along a NNE trend. One of the world&apos;s largest known Holocene explosive eruptions took place from Baitoushan about 1000 AD, depositing rhyolitic and trachytic tephra as far away as northern Japan and forming in part the present caldera.</obo:IAO_0000115>
        <oboInOwl:hasOBONamespace>GAZ</oboInOwl:hasOBONamespace>
        <oboInOwl:id>GAZ:00052993</oboInOwl:id>
        <rdfs:label>Baekdu Mountain</rdfs:label>
    </owl:NamedIndividual>
    


    <!-- http://purl.obolibrary.org/obo/GAZ_00052994 -->

    <owl:NamedIndividual rdf:about="http://purl.obolibrary.org/obo/GAZ_00052994">
        <obo:RO_0001025 rdf:resource="http://purl.obolibrary.org/obo/GAZ_00002801"/>
        <obo:IAO_0000115>A mountain in North Korea.</obo:IAO_0000115>
        <oboInOwl:hasOBONamespace>GAZ</oboInOwl:hasOBONamespace>
        <oboInOwl:id>GAZ:00052994</oboInOwl:id>
        <rdfs:label>Myohyang-san</rdfs:label>
    </owl:NamedIndividual>
    


    <!-- http://purl.obolibrary.org/obo/GAZ_00052995 -->

    <owl:NamedIndividual rdf:about="http://purl.obolibrary.org/obo/GAZ_00052995">
        <obo:RO_0001025 rdf:resource="http://purl.obolibrary.org/obo/GAZ_02000766"/>
        <oboInOwl:hasOBONamespace>GAZ</oboInOwl:hasOBONamespace>
        <oboInOwl:id>GAZ:00052995</oboInOwl:id>
        <rdfs:label>Mount Huchi Lyong</rdfs:label>
    </owl:NamedIndividual>
    


    <!-- http://purl.obolibrary.org/obo/GAZ_00052996 -->

    <owl:NamedIndividual rdf:about="http://purl.obolibrary.org/obo/GAZ_00052996">
        <obo:RO_0001025 rdf:resource="http://purl.obolibrary.org/obo/GAZ_00027814"/>
    </owl:NamedIndividual>
    


    <!-- http://purl.obolibrary.org/obo/GAZ_00054834 -->

    <owl:NamedIndividual rdf:about="http://purl.obolibrary.org/obo/GAZ_00054834">
        <obo:IAO_0000115>A mountain range on the border between China and North Korea. The range extends from the Northeast Chinese provinces of Jilin and Liaoning to the North Korean provinces of Ryanggang and Chagang. Most peaks exceed 2,000 m in height, with the highest mountain being Baekdu Mountain (Changbai Mountain).</obo:IAO_0000115>
        <oboInOwl:hasOBONamespace>GAZ</oboInOwl:hasOBONamespace>
        <oboInOwl:id>GAZ:00054834</oboInOwl:id>
        <rdfs:label>Baekdudaegan</rdfs:label>
    </owl:NamedIndividual>
    


    <!-- http://purl.obolibrary.org/obo/GAZ_00054837 -->

    <owl:NamedIndividual rdf:about="http://purl.obolibrary.org/obo/GAZ_00054837">
        <obo:RO_0001025 rdf:resource="http://purl.obolibrary.org/obo/GAZ_00054834"/>
        <obo:IAO_0000115>A little known volcano.</obo:IAO_0000115>
        <oboInOwl:hasOBONamespace>GAZ</oboInOwl:hasOBONamespace>
        <oboInOwl:id>GAZ:00054837</oboInOwl:id>
        <rdfs:label>Xianjindao Volcano</rdfs:label>
    </owl:NamedIndividual>
    


    <!-- http://purl.obolibrary.org/obo/GAZ_00054855 -->

    <owl:NamedIndividual rdf:about="http://purl.obolibrary.org/obo/GAZ_00054855">
        <obo:RO_0001025 rdf:resource="http://purl.obolibrary.org/obo/GAZ_00052993"/>
        <obo:IAO_0000115>A crater lake on the border between China and North Korea. It lies within a caldera atop the volcanic Baekdu Mountain, a part of the Baekdudaegan mountain range and the Changbai mountain range. It is located partly in Ryanggang Province, North Korea, and partly in Jilin Province, northeastern China.</obo:IAO_0000115>
        <oboInOwl:hasOBONamespace>GAZ</oboInOwl:hasOBONamespace>
        <oboInOwl:id>GAZ:00054855</oboInOwl:id>
        <rdfs:label>Tianchi Hu</rdfs:label>
    </owl:NamedIndividual>
    


    <!-- http://purl.obolibrary.org/obo/GAZ_00057402 -->

    <owl:NamedIndividual rdf:about="http://purl.obolibrary.org/obo/GAZ_00057402">
        <obo:IAO_0000115>A small outlying range of the Taebaek Mountains. They run along the east coast of South Korea through the cities of Pohang, Gyeongju, and Ulsan. The Dongdae Mountains separate the Hyeongsan River basin from the belt of small streams flowing directly into the Sea of Japan (East Sea).</obo:IAO_0000115>
        <oboInOwl:hasOBONamespace>GAZ</oboInOwl:hasOBONamespace>
        <oboInOwl:id>GAZ:00057402</oboInOwl:id>
        <rdfs:label>Dongdae Mountains</rdfs:label>
    </owl:NamedIndividual>
    


    <!-- http://purl.obolibrary.org/obo/GAZ_00057403 -->

    <owl:NamedIndividual rdf:about="http://purl.obolibrary.org/obo/GAZ_00057403">
        <obo:RO_0001025 rdf:resource="http://purl.obolibrary.org/obo/GAZ_00002801"/>
        <obo:IAO_0000115>A highland region of North Korea. It varies between 1,000 and 2,000 m in altitude and at 40,000 km2 is the largest tableland on the Korean Peninsula. It covers parts of the provinces of North and South Hamgyong, and North and South P&apos;yongan.</obo:IAO_0000115>
        <oboInOwl:hasOBONamespace>GAZ</oboInOwl:hasOBONamespace>
        <oboInOwl:id>GAZ:00057403</oboInOwl:id>
        <rdfs:label>Kaema Plateau</rdfs:label>
    </owl:NamedIndividual>
    


    <!-- http://purl.obolibrary.org/obo/GAZ_00057404 -->

    <owl:NamedIndividual rdf:about="http://purl.obolibrary.org/obo/GAZ_00057404">
        <obo:RO_0001025 rdf:resource="http://purl.obolibrary.org/obo/GAZ_00002801"/>
        <obo:RO_0001025 rdf:resource="http://purl.obolibrary.org/obo/GAZ_00027706"/>
        <obo:IAO_0000115>A mountain range stretching from north to south, west of the Kaema Highlands, in central North Korea. They are the source of several major rivers of North Korea, such as the Taedong and the Ch&apos;ongch&apos;on.</obo:IAO_0000115>
        <oboInOwl:hasOBONamespace>GAZ</oboInOwl:hasOBONamespace>
        <oboInOwl:id>GAZ:00057404</oboInOwl:id>
        <rdfs:label>Rangrim Mountains</rdfs:label>
    </owl:NamedIndividual>
    


    <!-- http://purl.obolibrary.org/obo/GAZ_00126554 -->

    <owl:NamedIndividual rdf:about="http://purl.obolibrary.org/obo/GAZ_00126554">
        <obo:RO_0001025 rdf:resource="http://purl.obolibrary.org/obo/GAZ_00054834"/>
        <obo:IAO_0000115>A mountain range cutting across the southern Korean peninsula. They split off from the Taebaek Mountains and trend southwest across the center of the peninsula. They are traditionally considered to reach their southwestern limit at Jiri-san, which is also the highest peak of the range. The Sobaek Mountains form the southern half of the Baekdudaegan. They mark the traditional border between the Honam and Yeongnam regions.</obo:IAO_0000115>
        <oboInOwl:hasOBONamespace>GAZ</oboInOwl:hasOBONamespace>
        <oboInOwl:id>GAZ:00126554</oboInOwl:id>
        <rdfs:label>Sobaek Mountains</rdfs:label>
    </owl:NamedIndividual>
    


    <!-- http://purl.obolibrary.org/obo/GAZ_00126869 -->

    <owl:NamedIndividual rdf:about="http://purl.obolibrary.org/obo/GAZ_00126869">
        <obo:RO_0001025 rdf:resource="http://purl.obolibrary.org/obo/GAZ_00126554"/>
        <obo:IAO_0000115>A national park.</obo:IAO_0000115>
        <oboInOwl:hasOBONamespace>GAZ</oboInOwl:hasOBONamespace>
        <oboInOwl:id>GAZ:00126869</oboInOwl:id>
        <rdfs:label>Songnisan National Park</rdfs:label>
    </owl:NamedIndividual>
    


    <!-- http://purl.obolibrary.org/obo/GAZ_00126877 -->

    <owl:NamedIndividual rdf:about="http://purl.obolibrary.org/obo/GAZ_00126877">
        <obo:RO_0001025 rdf:resource="http://purl.obolibrary.org/obo/GAZ_00126554"/>
        <obo:IAO_0000115>A national park.</obo:IAO_0000115>
        <oboInOwl:hasOBONamespace>GAZ</oboInOwl:hasOBONamespace>
        <oboInOwl:id>GAZ:00126877</oboInOwl:id>
        <rdfs:label>Woraksan National Park</rdfs:label>
    </owl:NamedIndividual>
    


    <!-- http://purl.obolibrary.org/obo/GAZ_00126878 -->

    <owl:NamedIndividual rdf:about="http://purl.obolibrary.org/obo/GAZ_00126878">
        <obo:RO_0001025 rdf:resource="http://purl.obolibrary.org/obo/GAZ_00126554"/>
        <obo:IAO_0000115>A national park.</obo:IAO_0000115>
        <oboInOwl:hasOBONamespace>GAZ</oboInOwl:hasOBONamespace>
        <oboInOwl:id>GAZ:00126878</oboInOwl:id>
        <rdfs:label>Sobaeksan National Park</rdfs:label>
    </owl:NamedIndividual>
    


    <!-- http://purl.obolibrary.org/obo/GAZ_00126928 -->

    <owl:NamedIndividual rdf:about="http://purl.obolibrary.org/obo/GAZ_00126928">
        <obo:RO_0001025 rdf:resource="http://purl.obolibrary.org/obo/GAZ_02000761"/>
        <obo:IAO_0000115>An island in Hwanghaenam Province.</obo:IAO_0000115>
        <oboInOwl:hasOBONamespace>GAZ</oboInOwl:hasOBONamespace>
        <oboInOwl:id>GAZ:00126928</oboInOwl:id>
        <rdfs:label>Sunwi-do</rdfs:label>
    </owl:NamedIndividual>
    


    <!-- http://purl.obolibrary.org/obo/GAZ_00126929 -->

    <owl:NamedIndividual rdf:about="http://purl.obolibrary.org/obo/GAZ_00126929">
        <obo:RO_0001025 rdf:resource="http://purl.obolibrary.org/obo/GAZ_02000761"/>
        <obo:IAO_0000115>An island in Hwanghaenam Province.</obo:IAO_0000115>
        <oboInOwl:hasOBONamespace>GAZ</oboInOwl:hasOBONamespace>
        <oboInOwl:id>GAZ:00126929</oboInOwl:id>
        <rdfs:label>Ch&apos;angnin-do</rdfs:label>
    </owl:NamedIndividual>
    


    <!-- http://purl.obolibrary.org/obo/GAZ_00126930 -->

    <owl:NamedIndividual rdf:about="http://purl.obolibrary.org/obo/GAZ_00126930">
        <obo:RO_0001025 rdf:resource="http://purl.obolibrary.org/obo/GAZ_02000761"/>
        <obo:IAO_0000115>An island in Hwanghaenam Province.</obo:IAO_0000115>
        <oboInOwl:hasOBONamespace>GAZ</oboInOwl:hasOBONamespace>
        <oboInOwl:id>GAZ:00126930</oboInOwl:id>
        <rdfs:label>Kirin-do</rdfs:label>
    </owl:NamedIndividual>
    


    <!-- http://purl.obolibrary.org/obo/GAZ_00128838 -->

    <owl:NamedIndividual rdf:about="http://purl.obolibrary.org/obo/GAZ_00128838">
        <obo:RO_0001025 rdf:resource="http://purl.obolibrary.org/obo/GAZ_00002801"/>
        <obo:RO_0001025 rdf:resource="http://purl.obolibrary.org/obo/GAZ_00027719"/>
        <obo:RO_0001025 rdf:resource="http://purl.obolibrary.org/obo/GAZ_00027726"/>
        <obo:RO_0001025 rdf:resource="http://purl.obolibrary.org/obo/GAZ_00027739"/>
        <obo:IAO_0000115>A mountain range of North Korea. They are located in the north-west of the country southeast of Sakchu.</obo:IAO_0000115>
        <oboInOwl:hasOBONamespace>GAZ</oboInOwl:hasOBONamespace>
        <oboInOwl:id>GAZ:00128838</oboInOwl:id>
        <rdfs:label>Kangnam Mountains</rdfs:label>
    </owl:NamedIndividual>
    


    <!-- http://purl.obolibrary.org/obo/GAZ_00128839 -->

    <owl:NamedIndividual rdf:about="http://purl.obolibrary.org/obo/GAZ_00128839">
        <obo:RO_0001025 rdf:resource="http://purl.obolibrary.org/obo/GAZ_00027704"/>
        <obo:IAO_0000115>A reservoir.</obo:IAO_0000115>
        <oboInOwl:hasOBONamespace>GAZ</oboInOwl:hasOBONamespace>
        <oboInOwl:id>GAZ:00128839</oboInOwl:id>
        <rdfs:label>Songwon Reservoir</rdfs:label>
    </owl:NamedIndividual>
    


    <!-- http://purl.obolibrary.org/obo/GAZ_00128840 -->

    <owl:NamedIndividual rdf:about="http://purl.obolibrary.org/obo/GAZ_00128840">
        <obo:RO_0001025 rdf:resource="http://purl.obolibrary.org/obo/GAZ_00027826"/>
        <obo:IAO_0000115>A ward of Ch&apos;ongjin City.</obo:IAO_0000115>
        <oboInOwl:hasOBONamespace>GAZ</oboInOwl:hasOBONamespace>
        <oboInOwl:id>GAZ:00128840</oboInOwl:id>
        <rdfs:label>Sunam-guyok</rdfs:label>
    </owl:NamedIndividual>
    


    <!-- http://purl.obolibrary.org/obo/GAZ_00128841 -->

    <owl:NamedIndividual rdf:about="http://purl.obolibrary.org/obo/GAZ_00128841">
        <obo:RO_0001025 rdf:resource="http://purl.obolibrary.org/obo/GAZ_00027826"/>
        <obo:IAO_0000115>A ward of Ch&apos;ongjin City.</obo:IAO_0000115>
        <oboInOwl:hasOBONamespace>GAZ</oboInOwl:hasOBONamespace>
        <oboInOwl:id>GAZ:00128841</oboInOwl:id>
        <rdfs:label>Songp&apos;yong-guyok</rdfs:label>
    </owl:NamedIndividual>
    


    <!-- http://purl.obolibrary.org/obo/GAZ_00128842 -->

    <owl:NamedIndividual rdf:about="http://purl.obolibrary.org/obo/GAZ_00128842">
        <obo:RO_0001025 rdf:resource="http://purl.obolibrary.org/obo/GAZ_00027826"/>
        <obo:IAO_0000115>A ward of Ch&apos;ongjin City.</obo:IAO_0000115>
        <oboInOwl:hasOBONamespace>GAZ</oboInOwl:hasOBONamespace>
        <oboInOwl:id>GAZ:00128842</oboInOwl:id>
        <rdfs:label>Ch&apos;ongam-guyok</rdfs:label>
    </owl:NamedIndividual>
    


    <!-- http://purl.obolibrary.org/obo/GAZ_00128843 -->

    <owl:NamedIndividual rdf:about="http://purl.obolibrary.org/obo/GAZ_00128843">
        <obo:RO_0001025 rdf:resource="http://purl.obolibrary.org/obo/GAZ_00027826"/>
        <obo:IAO_0000115>A ward of Ch&apos;ongjin City.</obo:IAO_0000115>
        <oboInOwl:hasOBONamespace>GAZ</oboInOwl:hasOBONamespace>
        <oboInOwl:id>GAZ:00128843</oboInOwl:id>
        <rdfs:label>P&apos;ohang-guyok</rdfs:label>
    </owl:NamedIndividual>
    


    <!-- http://purl.obolibrary.org/obo/GAZ_00128844 -->

    <owl:NamedIndividual rdf:about="http://purl.obolibrary.org/obo/GAZ_00128844">
        <obo:RO_0001025 rdf:resource="http://purl.obolibrary.org/obo/GAZ_00027826"/>
        <obo:IAO_0000115>A ward of Ch&apos;ongjin City.</obo:IAO_0000115>
        <oboInOwl:hasOBONamespace>GAZ</oboInOwl:hasOBONamespace>
        <oboInOwl:id>GAZ:00128844</oboInOwl:id>
        <rdfs:label>Ranam-guyok</rdfs:label>
    </owl:NamedIndividual>
    


    <!-- http://purl.obolibrary.org/obo/GAZ_00128845 -->

    <owl:NamedIndividual rdf:about="http://purl.obolibrary.org/obo/GAZ_00128845">
        <obo:RO_0001025 rdf:resource="http://purl.obolibrary.org/obo/GAZ_00027826"/>
        <obo:IAO_0000115>A ward of Ch&apos;ongjin City.</obo:IAO_0000115>
        <oboInOwl:hasOBONamespace>GAZ</oboInOwl:hasOBONamespace>
        <oboInOwl:id>GAZ:00128845</oboInOwl:id>
        <rdfs:label>Puyun-guyok</rdfs:label>
    </owl:NamedIndividual>
    


    <!-- http://purl.obolibrary.org/obo/GAZ_00128846 -->

    <owl:NamedIndividual rdf:about="http://purl.obolibrary.org/obo/GAZ_00128846">
        <obo:RO_0001025 rdf:resource="http://purl.obolibrary.org/obo/GAZ_00027826"/>
        <obo:IAO_0000115>A ward of Ch&apos;ongjin City.</obo:IAO_0000115>
        <oboInOwl:hasOBONamespace>GAZ</oboInOwl:hasOBONamespace>
        <oboInOwl:id>GAZ:00128846</oboInOwl:id>
        <rdfs:label>Sinam-guyok</rdfs:label>
    </owl:NamedIndividual>
    


    <!-- http://purl.obolibrary.org/obo/GAZ_00128847 -->

    <owl:NamedIndividual rdf:about="http://purl.obolibrary.org/obo/GAZ_00128847">
        <obo:RO_0001025 rdf:resource="http://purl.obolibrary.org/obo/GAZ_00027714"/>
        <obo:IAO_0000115>A mountain range in northeastern North Korea. The range forms a watershed that separates the northern frontier area along the Chinese border from the eastern Sea of Japan (East Sea) area. The Hamgyong Mountains lie on the northeastern edge of the Kaema Highlands and stretch southwest to the Pujollyong Mountains and northeast almost to the Tumen River.</obo:IAO_0000115>
        <oboInOwl:hasOBONamespace>GAZ</oboInOwl:hasOBONamespace>
        <oboInOwl:id>GAZ:00128847</oboInOwl:id>
        <rdfs:label>Hamgyong Mountains</rdfs:label>
    </owl:NamedIndividual>
    


    <!-- http://purl.obolibrary.org/obo/GAZ_00128848 -->

    <owl:NamedIndividual rdf:about="http://purl.obolibrary.org/obo/GAZ_00128848">
        <obo:RO_0001025 rdf:resource="http://purl.obolibrary.org/obo/GAZ_00002801"/>
        <obo:RO_0001025 rdf:resource="http://purl.obolibrary.org/obo/GAZ_00027686"/>
        <obo:RO_0001025 rdf:resource="http://purl.obolibrary.org/obo/GAZ_00027752"/>
        <obo:IAO_0000115>A mountain range which stretches from Mt. Paekdu forms a boundary between North and South Hamgyong provinces.</obo:IAO_0000115>
        <oboInOwl:hasOBONamespace>GAZ</oboInOwl:hasOBONamespace>
        <oboInOwl:id>GAZ:00128848</oboInOwl:id>
        <rdfs:label>Maryong Mountains</rdfs:label>
    </owl:NamedIndividual>
    


    <!-- http://purl.obolibrary.org/obo/GAZ_00128849 -->

    <owl:NamedIndividual rdf:about="http://purl.obolibrary.org/obo/GAZ_00128849">
        <obo:RO_0001025 rdf:resource="http://purl.obolibrary.org/obo/GAZ_00002801"/>
        <obo:RO_0001025 rdf:resource="http://purl.obolibrary.org/obo/GAZ_00027746"/>
        <obo:RO_0001025 rdf:resource="http://purl.obolibrary.org/obo/GAZ_00027752"/>
        <oboInOwl:hasOBONamespace>GAZ</oboInOwl:hasOBONamespace>
        <oboInOwl:id>GAZ:00128849</oboInOwl:id>
        <rdfs:label>Kwangju Mountains</rdfs:label>
    </owl:NamedIndividual>
    


    <!-- http://purl.obolibrary.org/obo/GAZ_00128850 -->

    <owl:NamedIndividual rdf:about="http://purl.obolibrary.org/obo/GAZ_00128850">
        <obo:RO_0001025 rdf:resource="http://purl.obolibrary.org/obo/GAZ_00027817"/>
        <obo:IAO_0000115>A brackish lake. It is fed by a branch of the Oranchon River.</obo:IAO_0000115>
        <oboInOwl:hasOBONamespace>GAZ</oboInOwl:hasOBONamespace>
        <oboInOwl:id>GAZ:00128850</oboInOwl:id>
        <rdfs:label>Mugye Lake</rdfs:label>
    </owl:NamedIndividual>
    


    <!-- http://purl.obolibrary.org/obo/GAZ_00128851 -->

    <owl:NamedIndividual rdf:about="http://purl.obolibrary.org/obo/GAZ_00128851">
        <obo:RO_0001025 rdf:resource="http://purl.obolibrary.org/obo/GAZ_00251690"/>
        <obo:IAO_0000115>A brackish lake. It is fed by a branch of the Oranchon River.</obo:IAO_0000115>
        <oboInOwl:hasOBONamespace>GAZ</oboInOwl:hasOBONamespace>
        <oboInOwl:id>GAZ:00128851</oboInOwl:id>
        <rdfs:label>Changyon Lake</rdfs:label>
    </owl:NamedIndividual>
    


    <!-- http://purl.obolibrary.org/obo/GAZ_00128852 -->

    <owl:NamedIndividual rdf:about="http://purl.obolibrary.org/obo/GAZ_00128852">
        <obo:RO_0001025 rdf:resource="http://purl.obolibrary.org/obo/GAZ_00002801"/>
        <oboInOwl:hasOBONamespace>GAZ</oboInOwl:hasOBONamespace>
        <oboInOwl:id>GAZ:00128852</oboInOwl:id>
        <rdfs:label>Paekmu Plateau</rdfs:label>
    </owl:NamedIndividual>
    


    <!-- http://purl.obolibrary.org/obo/GAZ_00128853 -->

    <owl:NamedIndividual rdf:about="http://purl.obolibrary.org/obo/GAZ_00128853">
        <obo:RO_0001025 rdf:resource="http://purl.obolibrary.org/obo/GAZ_00002801"/>
        <oboInOwl:hasOBONamespace>GAZ</oboInOwl:hasOBONamespace>
        <oboInOwl:id>GAZ:00128853</oboInOwl:id>
        <rdfs:label>Pujonryong Range</rdfs:label>
    </owl:NamedIndividual>
    


    <!-- http://purl.obolibrary.org/obo/GAZ_00128854 -->

    <owl:NamedIndividual rdf:about="http://purl.obolibrary.org/obo/GAZ_00128854">
        <obo:RO_0001025 rdf:resource="http://purl.obolibrary.org/obo/GAZ_00027764"/>
        <obo:RO_0001025 rdf:resource="http://purl.obolibrary.org/obo/GAZ_00128855"/>
        <obo:IAO_0000115>A dam on the Bukhan River, completed in 2003.</obo:IAO_0000115>
        <oboInOwl:hasOBONamespace>GAZ</oboInOwl:hasOBONamespace>
        <oboInOwl:id>GAZ:00128854</oboInOwl:id>
        <rdfs:label>Imnam Dam</rdfs:label>
    </owl:NamedIndividual>
    


    <!-- http://purl.obolibrary.org/obo/GAZ_00128855 -->

    <owl:NamedIndividual rdf:about="http://purl.obolibrary.org/obo/GAZ_00128855">
        <obo:RO_0001025 rdf:resource="http://purl.obolibrary.org/obo/GAZ_02000758"/>
        <obo:IAO_0000115>A river. A tributary of the Han River that flows through both North and South Korea. It traverses Kangwon province in North Korea and Gangwon and Gyeonggi provinces in South Korea. The Bukhan River&apos;s headwaters lie in North Korea near Geumgangsan; this early portion of the river is often called the Geumgangcheon. It crosses the Korean Demilitarized Zone and enters Hwacheon County, flowing south through Chuncheon and then west through Gapyeong. It joins with the Namhan River in Yangseo-myeon, Yangpyeong, to form the Han River.</obo:IAO_0000115>
        <oboInOwl:hasOBONamespace>GAZ</oboInOwl:hasOBONamespace>
        <oboInOwl:id>GAZ:00128855</oboInOwl:id>
        <rdfs:label>Bukhan River</rdfs:label>
    </owl:NamedIndividual>
    


    <!-- http://purl.obolibrary.org/obo/GAZ_00128856 -->

    <owl:NamedIndividual rdf:about="http://purl.obolibrary.org/obo/GAZ_00128856">
        <obo:RO_0001025 rdf:resource="http://purl.obolibrary.org/obo/GAZ_00002801"/>
        <obo:IAO_0000115>A river of North Korea. It flows from north to south, discharging to the Yellow Sea by Ganghwa Island, just west of the mouth of the River Imjin.</obo:IAO_0000115>
        <oboInOwl:hasOBONamespace>GAZ</oboInOwl:hasOBONamespace>
        <oboInOwl:id>GAZ:00128856</oboInOwl:id>
        <rdfs:label>Ryesong River</rdfs:label>
    </owl:NamedIndividual>
    


    <!-- http://purl.obolibrary.org/obo/GAZ_00128859 -->

    <owl:NamedIndividual rdf:about="http://purl.obolibrary.org/obo/GAZ_00128859">
        <obo:RO_0001025 rdf:resource="http://purl.obolibrary.org/obo/GAZ_02000760"/>
        <obo:RO_0001025 rdf:resource="http://purl.obolibrary.org/obo/GAZ_02000765"/>
        <obo:IAO_0000115>A river of North Korea having its source in the Rangrim Mountains of Chagang Province and discharging to the Yellow Sea at Sinanju. The river flows past Myohyang-san and through the city of Anju, South P&apos;yngan Province.</obo:IAO_0000115>
        <oboInOwl:hasOBONamespace>GAZ</oboInOwl:hasOBONamespace>
        <oboInOwl:id>GAZ:00128859</oboInOwl:id>
        <rdfs:label>Ch&apos;ongch&apos;on River</rdfs:label>
    </owl:NamedIndividual>
    


    <!-- http://purl.obolibrary.org/obo/GAZ_00128861 -->

    <owl:NamedIndividual rdf:about="http://purl.obolibrary.org/obo/GAZ_00128861">
        <obo:RO_0001025 rdf:resource="http://purl.obolibrary.org/obo/GAZ_00002801"/>
        <obo:IAO_0000115>The largest island in North Korea. It is situated in Korea Bay.</obo:IAO_0000115>
        <oboInOwl:hasOBONamespace>GAZ</oboInOwl:hasOBONamespace>
        <oboInOwl:id>GAZ:00128861</oboInOwl:id>
        <rdfs:label>Sinmi-do</rdfs:label>
    </owl:NamedIndividual>
    


    <!-- http://purl.obolibrary.org/obo/GAZ_00128862 -->

    <owl:NamedIndividual rdf:about="http://purl.obolibrary.org/obo/GAZ_00128862">
        <obo:RO_0001025 rdf:resource="http://purl.obolibrary.org/obo/GAZ_00027829"/>
        <obo:IAO_0000115>A &apos;worker&apos;s district&apos; of Onsong County.</obo:IAO_0000115>
        <oboInOwl:hasOBONamespace>GAZ</oboInOwl:hasOBONamespace>
        <oboInOwl:id>GAZ:00128862</oboInOwl:id>
        <rdfs:label>Sambong-rodongjagu</rdfs:label>
    </owl:NamedIndividual>
    


    <!-- http://purl.obolibrary.org/obo/GAZ_00128863 -->

    <owl:NamedIndividual rdf:about="http://purl.obolibrary.org/obo/GAZ_00128863">
        <obo:RO_0001025 rdf:resource="http://purl.obolibrary.org/obo/GAZ_00027829"/>
        <obo:IAO_0000115>A &apos;worker&apos;s district&apos; of Onsong County.</obo:IAO_0000115>
        <oboInOwl:hasOBONamespace>GAZ</oboInOwl:hasOBONamespace>
        <oboInOwl:id>GAZ:00128863</oboInOwl:id>
        <rdfs:label>Sansong-rodongjagu</rdfs:label>
    </owl:NamedIndividual>
    


    <!-- http://purl.obolibrary.org/obo/GAZ_00128864 -->

    <owl:NamedIndividual rdf:about="http://purl.obolibrary.org/obo/GAZ_00128864">
        <obo:RO_0001025 rdf:resource="http://purl.obolibrary.org/obo/GAZ_00027829"/>
        <obo:IAO_0000115>A &apos;worker&apos;s district&apos; of Onsong County.</obo:IAO_0000115>
        <oboInOwl:hasOBONamespace>GAZ</oboInOwl:hasOBONamespace>
        <oboInOwl:id>GAZ:00128864</oboInOwl:id>
        <rdfs:label>Sanghwa-rodongjagu</rdfs:label>
    </owl:NamedIndividual>
    


    <!-- http://purl.obolibrary.org/obo/GAZ_00128865 -->

    <owl:NamedIndividual rdf:about="http://purl.obolibrary.org/obo/GAZ_00128865">
        <obo:RO_0001025 rdf:resource="http://purl.obolibrary.org/obo/GAZ_00027829"/>
        <obo:IAO_0000115>A &apos;worker&apos;s district&apos; of Onsong County.</obo:IAO_0000115>
        <oboInOwl:hasOBONamespace>GAZ</oboInOwl:hasOBONamespace>
        <oboInOwl:id>GAZ:00128865</oboInOwl:id>
        <rdfs:label>Chuwon-rodongjagu</rdfs:label>
    </owl:NamedIndividual>
    


    <!-- http://purl.obolibrary.org/obo/GAZ_00128866 -->

    <owl:NamedIndividual rdf:about="http://purl.obolibrary.org/obo/GAZ_00128866">
        <obo:RO_0001025 rdf:resource="http://purl.obolibrary.org/obo/GAZ_00027829"/>
        <obo:IAO_0000115>A &apos;worker&apos;s district&apos; of Onsong County.</obo:IAO_0000115>
        <oboInOwl:hasOBONamespace>GAZ</oboInOwl:hasOBONamespace>
        <oboInOwl:id>GAZ:00128866</oboInOwl:id>
        <rdfs:label>Ontan-rodongjagu</rdfs:label>
    </owl:NamedIndividual>
    


    <!-- http://purl.obolibrary.org/obo/GAZ_00128867 -->

    <owl:NamedIndividual rdf:about="http://purl.obolibrary.org/obo/GAZ_00128867">
        <obo:RO_0001025 rdf:resource="http://purl.obolibrary.org/obo/GAZ_00027829"/>
        <obo:IAO_0000115>A &apos;worker&apos;s district&apos; of Onsong County.</obo:IAO_0000115>
        <oboInOwl:hasOBONamespace>GAZ</oboInOwl:hasOBONamespace>
        <oboInOwl:id>GAZ:00128867</oboInOwl:id>
        <rdfs:label>Changpyong-rodongjagu</rdfs:label>
    </owl:NamedIndividual>
    


    <!-- http://purl.obolibrary.org/obo/GAZ_00128868 -->

    <owl:NamedIndividual rdf:about="http://purl.obolibrary.org/obo/GAZ_00128868">
        <obo:RO_0001025 rdf:resource="http://purl.obolibrary.org/obo/GAZ_00027829"/>
        <obo:IAO_0000115>A &apos;worker&apos;s district&apos; of Onsong County.</obo:IAO_0000115>
        <oboInOwl:hasOBONamespace>GAZ</oboInOwl:hasOBONamespace>
        <oboInOwl:id>GAZ:00128868</oboInOwl:id>
        <rdfs:label>Chongsong-rodongjagu</rdfs:label>
    </owl:NamedIndividual>
    


    <!-- http://purl.obolibrary.org/obo/GAZ_00128869 -->

    <owl:NamedIndividual rdf:about="http://purl.obolibrary.org/obo/GAZ_00128869">
        <obo:RO_0001025 rdf:resource="http://purl.obolibrary.org/obo/GAZ_00027829"/>
        <obo:IAO_0000115>A &apos;worker&apos;s district&apos; of Onsong County.</obo:IAO_0000115>
        <oboInOwl:hasOBONamespace>GAZ</oboInOwl:hasOBONamespace>
        <oboInOwl:id>GAZ:00128869</oboInOwl:id>
        <rdfs:label>Pungin-rodongjagu</rdfs:label>
    </owl:NamedIndividual>
    


    <!-- http://purl.obolibrary.org/obo/GAZ_00128870 -->

    <owl:NamedIndividual rdf:about="http://purl.obolibrary.org/obo/GAZ_00128870">
        <obo:RO_0001025 rdf:resource="http://purl.obolibrary.org/obo/GAZ_00027829"/>
        <obo:IAO_0000115>A &apos;worker&apos;s district&apos; of Onsong County.</obo:IAO_0000115>
        <oboInOwl:hasOBONamespace>GAZ</oboInOwl:hasOBONamespace>
        <oboInOwl:id>GAZ:00128870</oboInOwl:id>
        <rdfs:label>Namyang-rodongjagu</rdfs:label>
    </owl:NamedIndividual>
    


    <!-- http://purl.obolibrary.org/obo/GAZ_00128871 -->

    <owl:NamedIndividual rdf:about="http://purl.obolibrary.org/obo/GAZ_00128871">
        <obo:RO_0001025 rdf:resource="http://purl.obolibrary.org/obo/GAZ_00027829"/>
        <obo:IAO_0000115>A &apos;worker&apos;s district&apos; of Onsong County.</obo:IAO_0000115>
        <oboInOwl:hasOBONamespace>GAZ</oboInOwl:hasOBONamespace>
        <oboInOwl:id>GAZ:00128871</oboInOwl:id>
        <rdfs:label>Tongpo-rodongjagu</rdfs:label>
    </owl:NamedIndividual>
    


    <!-- http://purl.obolibrary.org/obo/GAZ_00128872 -->

    <owl:NamedIndividual rdf:about="http://purl.obolibrary.org/obo/GAZ_00128872">
        <rdf:type rdf:resource="http://purl.obolibrary.org/obo/ENVO_00000856"/>
        <obo:RO_0001025 rdf:resource="http://purl.obolibrary.org/obo/GAZ_00027829"/>
        <obo:IAO_0000115>A populated place. A town of Onsong County.</obo:IAO_0000115>
        <oboInOwl:hasOBONamespace>GAZ</oboInOwl:hasOBONamespace>
        <oboInOwl:id>GAZ:00128872</oboInOwl:id>
        <rdfs:label>Onsong-up</rdfs:label>
    </owl:NamedIndividual>
    


    <!-- http://purl.obolibrary.org/obo/GAZ_00128873 -->

    <owl:NamedIndividual rdf:about="http://purl.obolibrary.org/obo/GAZ_00128873">
        <rdf:type rdf:resource="http://purl.obolibrary.org/obo/ENVO_00000856"/>
        <obo:RO_0001025 rdf:resource="http://purl.obolibrary.org/obo/GAZ_00027829"/>
        <obo:IAO_0000115>A populated place. A village of Onsong County.</obo:IAO_0000115>
        <oboInOwl:hasOBONamespace>GAZ</oboInOwl:hasOBONamespace>
        <oboInOwl:id>GAZ:00128873</oboInOwl:id>
        <rdfs:label>Pungso-ri</rdfs:label>
    </owl:NamedIndividual>
    


    <!-- http://purl.obolibrary.org/obo/GAZ_00128874 -->

    <owl:NamedIndividual rdf:about="http://purl.obolibrary.org/obo/GAZ_00128874">
        <rdf:type rdf:resource="http://purl.obolibrary.org/obo/ENVO_00000856"/>
        <obo:RO_0001025 rdf:resource="http://purl.obolibrary.org/obo/GAZ_00027829"/>
        <obo:IAO_0000115>A populated place. A village of Onsong County.</obo:IAO_0000115>
        <oboInOwl:hasOBONamespace>GAZ</oboInOwl:hasOBONamespace>
        <oboInOwl:id>GAZ:00128874</oboInOwl:id>
        <rdfs:label>Pungha-ri</rdfs:label>
    </owl:NamedIndividual>
    


    <!-- http://purl.obolibrary.org/obo/GAZ_00128875 -->

    <owl:NamedIndividual rdf:about="http://purl.obolibrary.org/obo/GAZ_00128875">
        <rdf:type rdf:resource="http://purl.obolibrary.org/obo/ENVO_00000856"/>
        <obo:RO_0001025 rdf:resource="http://purl.obolibrary.org/obo/GAZ_00027829"/>
        <obo:IAO_0000115>A populated place. A village of Onsong County.</obo:IAO_0000115>
        <oboInOwl:hasOBONamespace>GAZ</oboInOwl:hasOBONamespace>
        <oboInOwl:id>GAZ:00128875</oboInOwl:id>
        <rdfs:label>Pungchon-ri</rdfs:label>
    </owl:NamedIndividual>
    


    <!-- http://purl.obolibrary.org/obo/GAZ_00128876 -->

    <owl:NamedIndividual rdf:about="http://purl.obolibrary.org/obo/GAZ_00128876">
        <rdf:type rdf:resource="http://purl.obolibrary.org/obo/ENVO_00000856"/>
        <obo:RO_0001025 rdf:resource="http://purl.obolibrary.org/obo/GAZ_00027829"/>
        <obo:IAO_0000115>A populated place. A village of Onsong County.</obo:IAO_0000115>
        <oboInOwl:hasOBONamespace>GAZ</oboInOwl:hasOBONamespace>
        <oboInOwl:id>GAZ:00128876</oboInOwl:id>
        <rdfs:label>Hasambong-ri</rdfs:label>
    </owl:NamedIndividual>
    


    <!-- http://purl.obolibrary.org/obo/GAZ_00128877 -->

    <owl:NamedIndividual rdf:about="http://purl.obolibrary.org/obo/GAZ_00128877">
        <rdf:type rdf:resource="http://purl.obolibrary.org/obo/ENVO_00000856"/>
        <obo:RO_0001025 rdf:resource="http://purl.obolibrary.org/obo/GAZ_00027829"/>
        <obo:IAO_0000115>A populated place. A village of Onsong County.</obo:IAO_0000115>
        <oboInOwl:hasOBONamespace>GAZ</oboInOwl:hasOBONamespace>
        <oboInOwl:id>GAZ:00128877</oboInOwl:id>
        <rdfs:label>Chungsan-ri</rdfs:label>
    </owl:NamedIndividual>
    


    <!-- http://purl.obolibrary.org/obo/GAZ_00128878 -->

    <owl:NamedIndividual rdf:about="http://purl.obolibrary.org/obo/GAZ_00128878">
        <rdf:type rdf:resource="http://purl.obolibrary.org/obo/ENVO_00000856"/>
        <obo:RO_0001025 rdf:resource="http://purl.obolibrary.org/obo/GAZ_00027829"/>
        <obo:IAO_0000115>A populated place. A village of Onsong County.</obo:IAO_0000115>
        <oboInOwl:hasOBONamespace>GAZ</oboInOwl:hasOBONamespace>
        <oboInOwl:id>GAZ:00128878</oboInOwl:id>
        <rdfs:label>Wangjaesan-ri</rdfs:label>
    </owl:NamedIndividual>
    


    <!-- http://purl.obolibrary.org/obo/GAZ_00128879 -->

    <owl:NamedIndividual rdf:about="http://purl.obolibrary.org/obo/GAZ_00128879">
        <rdf:type rdf:resource="http://purl.obolibrary.org/obo/ENVO_00000856"/>
        <obo:RO_0001025 rdf:resource="http://purl.obolibrary.org/obo/GAZ_00027829"/>
        <obo:IAO_0000115>A populated place. A village of Onsong County.</obo:IAO_0000115>
        <oboInOwl:hasOBONamespace>GAZ</oboInOwl:hasOBONamespace>
        <oboInOwl:id>GAZ:00128879</oboInOwl:id>
        <rdfs:label>Yonggang-ri</rdfs:label>
    </owl:NamedIndividual>
    


    <!-- http://purl.obolibrary.org/obo/GAZ_00128880 -->

    <owl:NamedIndividual rdf:about="http://purl.obolibrary.org/obo/GAZ_00128880">
        <rdf:type rdf:resource="http://purl.obolibrary.org/obo/ENVO_00000856"/>
        <obo:RO_0001025 rdf:resource="http://purl.obolibrary.org/obo/GAZ_00027829"/>
        <obo:IAO_0000115>A populated place. A village of Onsong County.</obo:IAO_0000115>
        <oboInOwl:hasOBONamespace>GAZ</oboInOwl:hasOBONamespace>
        <oboInOwl:id>GAZ:00128880</oboInOwl:id>
        <rdfs:label>Punggye-ri</rdfs:label>
    </owl:NamedIndividual>
    


    <!-- http://purl.obolibrary.org/obo/GAZ_00128881 -->

    <owl:NamedIndividual rdf:about="http://purl.obolibrary.org/obo/GAZ_00128881">
        <rdf:type rdf:resource="http://purl.obolibrary.org/obo/ENVO_00000856"/>
        <obo:RO_0001025 rdf:resource="http://purl.obolibrary.org/obo/GAZ_00027829"/>
        <obo:IAO_0000115>A populated place. A village of Onsong County.</obo:IAO_0000115>
        <oboInOwl:hasOBONamespace>GAZ</oboInOwl:hasOBONamespace>
        <oboInOwl:id>GAZ:00128881</oboInOwl:id>
        <rdfs:label>Unam-ri</rdfs:label>
    </owl:NamedIndividual>
    


    <!-- http://purl.obolibrary.org/obo/GAZ_00128882 -->

    <owl:NamedIndividual rdf:about="http://purl.obolibrary.org/obo/GAZ_00128882">
        <rdf:type rdf:resource="http://purl.obolibrary.org/obo/ENVO_00000856"/>
        <obo:RO_0001025 rdf:resource="http://purl.obolibrary.org/obo/GAZ_00027829"/>
        <obo:IAO_0000115>A populated place. A village of Onsong County.</obo:IAO_0000115>
        <oboInOwl:hasOBONamespace>GAZ</oboInOwl:hasOBONamespace>
        <oboInOwl:id>GAZ:00128882</oboInOwl:id>
        <rdfs:label>Kangan-ri</rdfs:label>
    </owl:NamedIndividual>
    


    <!-- http://purl.obolibrary.org/obo/GAZ_00128883 -->

    <owl:NamedIndividual rdf:about="http://purl.obolibrary.org/obo/GAZ_00128883">
        <rdf:type rdf:resource="http://purl.obolibrary.org/obo/ENVO_00000856"/>
        <obo:RO_0001025 rdf:resource="http://purl.obolibrary.org/obo/GAZ_00027829"/>
        <obo:IAO_0000115>A populated place. A village of Onsong County.</obo:IAO_0000115>
        <oboInOwl:hasOBONamespace>GAZ</oboInOwl:hasOBONamespace>
        <oboInOwl:id>GAZ:00128883</oboInOwl:id>
        <rdfs:label>Seson-ri</rdfs:label>
    </owl:NamedIndividual>
    


    <!-- http://purl.obolibrary.org/obo/GAZ_00128884 -->

    <owl:NamedIndividual rdf:about="http://purl.obolibrary.org/obo/GAZ_00128884">
        <rdf:type rdf:resource="http://purl.obolibrary.org/obo/ENVO_00000856"/>
        <obo:RO_0001025 rdf:resource="http://purl.obolibrary.org/obo/GAZ_00027829"/>
        <obo:IAO_0000115>A populated place. A village of Onsong County.</obo:IAO_0000115>
        <oboInOwl:hasOBONamespace>GAZ</oboInOwl:hasOBONamespace>
        <oboInOwl:id>GAZ:00128884</oboInOwl:id>
        <rdfs:label>Hyangdang-ri</rdfs:label>
    </owl:NamedIndividual>
    


    <!-- http://purl.obolibrary.org/obo/GAZ_00128885 -->

    <owl:NamedIndividual rdf:about="http://purl.obolibrary.org/obo/GAZ_00128885">
        <rdf:type rdf:resource="http://purl.obolibrary.org/obo/ENVO_00000856"/>
        <obo:RO_0001025 rdf:resource="http://purl.obolibrary.org/obo/GAZ_00027829"/>
        <obo:IAO_0000115>A populated place. A village of Onsong County.</obo:IAO_0000115>
        <oboInOwl:hasOBONamespace>GAZ</oboInOwl:hasOBONamespace>
        <oboInOwl:id>GAZ:00128885</oboInOwl:id>
        <rdfs:label>Misan-ri</rdfs:label>
    </owl:NamedIndividual>
    


    <!-- http://purl.obolibrary.org/obo/GAZ_00128886 -->

    <owl:NamedIndividual rdf:about="http://purl.obolibrary.org/obo/GAZ_00128886">
        <rdf:type rdf:resource="http://purl.obolibrary.org/obo/ENVO_00000856"/>
        <obo:RO_0001025 rdf:resource="http://purl.obolibrary.org/obo/GAZ_00027829"/>
        <obo:IAO_0000115>A populated place. A village of Onsong County.</obo:IAO_0000115>
        <oboInOwl:hasOBONamespace>GAZ</oboInOwl:hasOBONamespace>
        <oboInOwl:id>GAZ:00128886</oboInOwl:id>
        <rdfs:label>Ryongnam-ri</rdfs:label>
    </owl:NamedIndividual>
    


    <!-- http://purl.obolibrary.org/obo/GAZ_00128887 -->

    <owl:NamedIndividual rdf:about="http://purl.obolibrary.org/obo/GAZ_00128887">
        <rdf:type rdf:resource="http://purl.obolibrary.org/obo/ENVO_00000856"/>
        <obo:RO_0001025 rdf:resource="http://purl.obolibrary.org/obo/GAZ_00027829"/>
        <obo:IAO_0000115>A populated place. A village of Onsong County.</obo:IAO_0000115>
        <oboInOwl:hasOBONamespace>GAZ</oboInOwl:hasOBONamespace>
        <oboInOwl:id>GAZ:00128887</oboInOwl:id>
        <rdfs:label>Tulubong-ri</rdfs:label>
    </owl:NamedIndividual>
    


    <!-- http://purl.obolibrary.org/obo/GAZ_00128888 -->

    <owl:NamedIndividual rdf:about="http://purl.obolibrary.org/obo/GAZ_00128888">
        <rdf:type rdf:resource="http://purl.obolibrary.org/obo/ENVO_00000856"/>
        <obo:RO_0001025 rdf:resource="http://purl.obolibrary.org/obo/GAZ_00027828"/>
        <obo:IAO_0000115>A populated place. A town of Saebyol County.</obo:IAO_0000115>
        <oboInOwl:hasOBONamespace>GAZ</oboInOwl:hasOBONamespace>
        <oboInOwl:id>GAZ:00128888</oboInOwl:id>
        <rdfs:label>Saebyol-up</rdfs:label>
    </owl:NamedIndividual>
    


    <!-- http://purl.obolibrary.org/obo/GAZ_00128889 -->

    <owl:NamedIndividual rdf:about="http://purl.obolibrary.org/obo/GAZ_00128889">
        <obo:RO_0001025 rdf:resource="http://purl.obolibrary.org/obo/GAZ_00027828"/>
        <obo:IAO_0000115>A &apos;worker&apos;s district&apos; of Saebyol County.</obo:IAO_0000115>
        <oboInOwl:hasOBONamespace>GAZ</oboInOwl:hasOBONamespace>
        <oboInOwl:id>GAZ:00128889</oboInOwl:id>
        <rdfs:label>Hamyon-rodongjagu</rdfs:label>
    </owl:NamedIndividual>
    


    <!-- http://purl.obolibrary.org/obo/GAZ_00128890 -->

    <owl:NamedIndividual rdf:about="http://purl.obolibrary.org/obo/GAZ_00128890">
        <obo:RO_0001025 rdf:resource="http://purl.obolibrary.org/obo/GAZ_00027828"/>
        <obo:IAO_0000115>A &apos;worker&apos;s district&apos; of Saebyol County.</obo:IAO_0000115>
        <oboInOwl:hasOBONamespace>GAZ</oboInOwl:hasOBONamespace>
        <oboInOwl:id>GAZ:00128890</oboInOwl:id>
        <rdfs:label>Ryongbuk-rodongjagu</rdfs:label>
    </owl:NamedIndividual>
    


    <!-- http://purl.obolibrary.org/obo/GAZ_00128891 -->

    <owl:NamedIndividual rdf:about="http://purl.obolibrary.org/obo/GAZ_00128891">
        <obo:RO_0001025 rdf:resource="http://purl.obolibrary.org/obo/GAZ_00027828"/>
        <obo:IAO_0000115>A &apos;worker&apos;s district&apos; of Saebyol County.</obo:IAO_0000115>
        <oboInOwl:hasOBONamespace>GAZ</oboInOwl:hasOBONamespace>
        <oboInOwl:id>GAZ:00128891</oboInOwl:id>
        <rdfs:label>Kogonwon-rodongjagu</rdfs:label>
    </owl:NamedIndividual>
    


    <!-- http://purl.obolibrary.org/obo/GAZ_00128892 -->

    <owl:NamedIndividual rdf:about="http://purl.obolibrary.org/obo/GAZ_00128892">
        <rdf:type rdf:resource="http://purl.obolibrary.org/obo/ENVO_00000856"/>
        <obo:RO_0001025 rdf:resource="http://purl.obolibrary.org/obo/GAZ_00027828"/>
        <obo:IAO_0000115>A populated place. A village of Saebyol County.</obo:IAO_0000115>
        <oboInOwl:hasOBONamespace>GAZ</oboInOwl:hasOBONamespace>
        <oboInOwl:id>GAZ:00128892</oboInOwl:id>
        <rdfs:label>Chungyong-ri</rdfs:label>
    </owl:NamedIndividual>
    


    <!-- http://purl.obolibrary.org/obo/GAZ_00128893 -->

    <owl:NamedIndividual rdf:about="http://purl.obolibrary.org/obo/GAZ_00128893">
        <rdf:type rdf:resource="http://purl.obolibrary.org/obo/ENVO_00000856"/>
        <obo:RO_0001025 rdf:resource="http://purl.obolibrary.org/obo/GAZ_00027828"/>
        <obo:IAO_0000115>A populated place. A village of Saebyol County.</obo:IAO_0000115>
        <oboInOwl:hasOBONamespace>GAZ</oboInOwl:hasOBONamespace>
        <oboInOwl:id>GAZ:00128893</oboInOwl:id>
        <rdfs:label>Yonsan-ri</rdfs:label>
    </owl:NamedIndividual>
    


    <!-- http://purl.obolibrary.org/obo/GAZ_00128894 -->

    <owl:NamedIndividual rdf:about="http://purl.obolibrary.org/obo/GAZ_00128894">
        <rdf:type rdf:resource="http://purl.obolibrary.org/obo/ENVO_00000856"/>
        <obo:RO_0001025 rdf:resource="http://purl.obolibrary.org/obo/GAZ_00027828"/>
        <obo:IAO_0000115>A populated place. A village of Saebyol County.</obo:IAO_0000115>
        <oboInOwl:hasOBONamespace>GAZ</oboInOwl:hasOBONamespace>
        <oboInOwl:id>GAZ:00128894</oboInOwl:id>
        <rdfs:label>Songnae-ri</rdfs:label>
    </owl:NamedIndividual>
    


    <!-- http://purl.obolibrary.org/obo/GAZ_00128895 -->

    <owl:NamedIndividual rdf:about="http://purl.obolibrary.org/obo/GAZ_00128895">
        <rdf:type rdf:resource="http://purl.obolibrary.org/obo/ENVO_00000856"/>
        <obo:RO_0001025 rdf:resource="http://purl.obolibrary.org/obo/GAZ_00027828"/>
        <obo:IAO_0000115>A populated place. A village of Saebyol County.</obo:IAO_0000115>
        <oboInOwl:hasOBONamespace>GAZ</oboInOwl:hasOBONamespace>
        <oboInOwl:id>GAZ:00128895</oboInOwl:id>
        <rdfs:label>Anwon-ri</rdfs:label>
    </owl:NamedIndividual>
    


    <!-- http://purl.obolibrary.org/obo/GAZ_00128896 -->

    <owl:NamedIndividual rdf:about="http://purl.obolibrary.org/obo/GAZ_00128896">
        <rdf:type rdf:resource="http://purl.obolibrary.org/obo/ENVO_00000856"/>
        <obo:RO_0001025 rdf:resource="http://purl.obolibrary.org/obo/GAZ_00027828"/>
        <obo:IAO_0000115>A populated place. A village of Saebyol County.</obo:IAO_0000115>
        <oboInOwl:hasOBONamespace>GAZ</oboInOwl:hasOBONamespace>
        <oboInOwl:id>GAZ:00128896</oboInOwl:id>
        <rdfs:label>Ryongdang-ri</rdfs:label>
    </owl:NamedIndividual>
    


    <!-- http://purl.obolibrary.org/obo/GAZ_00128897 -->

    <owl:NamedIndividual rdf:about="http://purl.obolibrary.org/obo/GAZ_00128897">
        <rdf:type rdf:resource="http://purl.obolibrary.org/obo/ENVO_00000856"/>
        <obo:RO_0001025 rdf:resource="http://purl.obolibrary.org/obo/GAZ_00027828"/>
        <obo:IAO_0000115>A populated place. A village of Saebyol County.</obo:IAO_0000115>
        <oboInOwl:hasOBONamespace>GAZ</oboInOwl:hasOBONamespace>
        <oboInOwl:id>GAZ:00128897</oboInOwl:id>
        <rdfs:label>Ryonggye-ri</rdfs:label>
    </owl:NamedIndividual>
    


    <!-- http://purl.obolibrary.org/obo/GAZ_00128898 -->

    <owl:NamedIndividual rdf:about="http://purl.obolibrary.org/obo/GAZ_00128898">
        <rdf:type rdf:resource="http://purl.obolibrary.org/obo/ENVO_00000856"/>
        <obo:RO_0001025 rdf:resource="http://purl.obolibrary.org/obo/GAZ_00027828"/>
        <obo:IAO_0000115>A populated place. A village of Saebyol County.</obo:IAO_0000115>
        <oboInOwl:hasOBONamespace>GAZ</oboInOwl:hasOBONamespace>
        <oboInOwl:id>GAZ:00128898</oboInOwl:id>
        <rdfs:label>Bongsan-ri</rdfs:label>
    </owl:NamedIndividual>
    


    <!-- http://purl.obolibrary.org/obo/GAZ_00128899 -->

    <owl:NamedIndividual rdf:about="http://purl.obolibrary.org/obo/GAZ_00128899">
        <rdf:type rdf:resource="http://purl.obolibrary.org/obo/ENVO_00000856"/>
        <obo:RO_0001025 rdf:resource="http://purl.obolibrary.org/obo/GAZ_00027828"/>
        <obo:IAO_0000115>A populated place. A village of Saebyol County.</obo:IAO_0000115>
        <oboInOwl:hasOBONamespace>GAZ</oboInOwl:hasOBONamespace>
        <oboInOwl:id>GAZ:00128899</oboInOwl:id>
        <rdfs:label>Kumdong-ri</rdfs:label>
    </owl:NamedIndividual>
    


    <!-- http://purl.obolibrary.org/obo/GAZ_00128900 -->

    <owl:NamedIndividual rdf:about="http://purl.obolibrary.org/obo/GAZ_00128900">
        <rdf:type rdf:resource="http://purl.obolibrary.org/obo/ENVO_00000856"/>
        <obo:RO_0001025 rdf:resource="http://purl.obolibrary.org/obo/GAZ_00027828"/>
        <obo:IAO_0000115>A populated place. A village of Saebyol County.</obo:IAO_0000115>
        <oboInOwl:hasOBONamespace>GAZ</oboInOwl:hasOBONamespace>
        <oboInOwl:id>GAZ:00128900</oboInOwl:id>
        <rdfs:label>Nongpo-ri</rdfs:label>
    </owl:NamedIndividual>
    


    <!-- http://purl.obolibrary.org/obo/GAZ_00128901 -->

    <owl:NamedIndividual rdf:about="http://purl.obolibrary.org/obo/GAZ_00128901">
        <rdf:type rdf:resource="http://purl.obolibrary.org/obo/ENVO_00000856"/>
        <obo:RO_0001025 rdf:resource="http://purl.obolibrary.org/obo/GAZ_00027828"/>
        <obo:IAO_0000115>A populated place. A village of Saebyol County.</obo:IAO_0000115>
        <oboInOwl:hasOBONamespace>GAZ</oboInOwl:hasOBONamespace>
        <oboInOwl:id>GAZ:00128901</oboInOwl:id>
        <rdfs:label>Tongrim-ri</rdfs:label>
    </owl:NamedIndividual>
    


    <!-- http://purl.obolibrary.org/obo/GAZ_00128902 -->

    <owl:NamedIndividual rdf:about="http://purl.obolibrary.org/obo/GAZ_00128902">
        <rdf:type rdf:resource="http://purl.obolibrary.org/obo/ENVO_00000856"/>
        <obo:RO_0001025 rdf:resource="http://purl.obolibrary.org/obo/GAZ_00027828"/>
        <obo:IAO_0000115>A populated place. A village of Saebyol County.</obo:IAO_0000115>
        <oboInOwl:hasOBONamespace>GAZ</oboInOwl:hasOBONamespace>
        <oboInOwl:id>GAZ:00128902</oboInOwl:id>
        <rdfs:label>Chongsan-ri</rdfs:label>
    </owl:NamedIndividual>
    


    <!-- http://purl.obolibrary.org/obo/GAZ_00128903 -->

    <owl:NamedIndividual rdf:about="http://purl.obolibrary.org/obo/GAZ_00128903">
        <rdf:type rdf:resource="http://purl.obolibrary.org/obo/ENVO_00000856"/>
        <obo:RO_0001025 rdf:resource="http://purl.obolibrary.org/obo/GAZ_00027828"/>
        <obo:IAO_0000115>A populated place. A village of Saebyol County.</obo:IAO_0000115>
        <oboInOwl:hasOBONamespace>GAZ</oboInOwl:hasOBONamespace>
        <oboInOwl:id>GAZ:00128903</oboInOwl:id>
        <rdfs:label>Ryongmun-ri</rdfs:label>
    </owl:NamedIndividual>
    


    <!-- http://purl.obolibrary.org/obo/GAZ_00128904 -->

    <owl:NamedIndividual rdf:about="http://purl.obolibrary.org/obo/GAZ_00128904">
        <rdf:type rdf:resource="http://purl.obolibrary.org/obo/ENVO_00000856"/>
        <obo:RO_0001025 rdf:resource="http://purl.obolibrary.org/obo/GAZ_00027828"/>
        <obo:IAO_0000115>A populated place. A village of Saebyol County.</obo:IAO_0000115>
        <oboInOwl:hasOBONamespace>GAZ</oboInOwl:hasOBONamespace>
        <oboInOwl:id>GAZ:00128904</oboInOwl:id>
        <rdfs:label>Sasu-ri</rdfs:label>
    </owl:NamedIndividual>
    


    <!-- http://purl.obolibrary.org/obo/GAZ_00128905 -->

    <owl:NamedIndividual rdf:about="http://purl.obolibrary.org/obo/GAZ_00128905">
        <rdf:type rdf:resource="http://purl.obolibrary.org/obo/ENVO_00000856"/>
        <obo:RO_0001025 rdf:resource="http://purl.obolibrary.org/obo/GAZ_00027828"/>
        <obo:IAO_0000115>A populated place. A village of Saebyol County.</obo:IAO_0000115>
        <oboInOwl:hasOBONamespace>GAZ</oboInOwl:hasOBONamespace>
        <oboInOwl:id>GAZ:00128905</oboInOwl:id>
        <rdfs:label>Ryongsin-ri</rdfs:label>
    </owl:NamedIndividual>
    


    <!-- http://purl.obolibrary.org/obo/GAZ_00128906 -->

    <owl:NamedIndividual rdf:about="http://purl.obolibrary.org/obo/GAZ_00128906">
        <rdf:type rdf:resource="http://purl.obolibrary.org/obo/ENVO_00000856"/>
        <obo:RO_0001025 rdf:resource="http://purl.obolibrary.org/obo/GAZ_00027828"/>
        <obo:IAO_0000115>A populated place. A village of Saebyol County.</obo:IAO_0000115>
        <oboInOwl:hasOBONamespace>GAZ</oboInOwl:hasOBONamespace>
        <oboInOwl:id>GAZ:00128906</oboInOwl:id>
        <rdfs:label>Ryongnam-ri</rdfs:label>
    </owl:NamedIndividual>
    


    <!-- http://purl.obolibrary.org/obo/GAZ_00128907 -->

    <owl:NamedIndividual rdf:about="http://purl.obolibrary.org/obo/GAZ_00128907">
        <rdf:type rdf:resource="http://purl.obolibrary.org/obo/ENVO_00000856"/>
        <obo:RO_0001025 rdf:resource="http://purl.obolibrary.org/obo/GAZ_00027828"/>
        <obo:IAO_0000115>A populated place. A village of Saebyol County.</obo:IAO_0000115>
        <oboInOwl:hasOBONamespace>GAZ</oboInOwl:hasOBONamespace>
        <oboInOwl:id>GAZ:00128907</oboInOwl:id>
        <rdfs:label>Singon-ri</rdfs:label>
    </owl:NamedIndividual>
    


    <!-- http://purl.obolibrary.org/obo/GAZ_00128908 -->

    <owl:NamedIndividual rdf:about="http://purl.obolibrary.org/obo/GAZ_00128908">
        <rdf:type rdf:resource="http://purl.obolibrary.org/obo/ENVO_00000856"/>
        <obo:RO_0001025 rdf:resource="http://purl.obolibrary.org/obo/GAZ_00027828"/>
        <obo:IAO_0000115>A populated place. A village of Saebyol County.</obo:IAO_0000115>
        <oboInOwl:hasOBONamespace>GAZ</oboInOwl:hasOBONamespace>
        <oboInOwl:id>GAZ:00128908</oboInOwl:id>
        <rdfs:label>Ryudasom-ri</rdfs:label>
    </owl:NamedIndividual>
    


    <!-- http://purl.obolibrary.org/obo/GAZ_00128909 -->

    <owl:NamedIndividual rdf:about="http://purl.obolibrary.org/obo/GAZ_00128909">
        <rdf:type rdf:resource="http://purl.obolibrary.org/obo/ENVO_00000856"/>
        <obo:RO_0001025 rdf:resource="http://purl.obolibrary.org/obo/GAZ_00027828"/>
        <obo:IAO_0000115>A populated place. A village of Saebyol County.</obo:IAO_0000115>
        <oboInOwl:hasOBONamespace>GAZ</oboInOwl:hasOBONamespace>
        <oboInOwl:id>GAZ:00128909</oboInOwl:id>
        <rdfs:label>Hunyung-ri</rdfs:label>
    </owl:NamedIndividual>
    


    <!-- http://purl.obolibrary.org/obo/GAZ_00128910 -->

    <owl:NamedIndividual rdf:about="http://purl.obolibrary.org/obo/GAZ_00128910">
        <rdf:type rdf:resource="http://purl.obolibrary.org/obo/ENVO_00000856"/>
        <obo:RO_0001025 rdf:resource="http://purl.obolibrary.org/obo/GAZ_00027828"/>
        <obo:IAO_0000115>A populated place. A village of Saebyol County.</obo:IAO_0000115>
        <oboInOwl:hasOBONamespace>GAZ</oboInOwl:hasOBONamespace>
        <oboInOwl:id>GAZ:00128910</oboInOwl:id>
        <rdfs:label>Ryonghyon-ri</rdfs:label>
    </owl:NamedIndividual>
    


    <!-- http://purl.obolibrary.org/obo/GAZ_00128911 -->

    <owl:NamedIndividual rdf:about="http://purl.obolibrary.org/obo/GAZ_00128911">
        <rdf:type rdf:resource="http://purl.obolibrary.org/obo/ENVO_00000856"/>
        <obo:RO_0001025 rdf:resource="http://purl.obolibrary.org/obo/GAZ_00027828"/>
        <obo:IAO_0000115>A populated place. A village of Saebyol County.</obo:IAO_0000115>
        <oboInOwl:hasOBONamespace>GAZ</oboInOwl:hasOBONamespace>
        <oboInOwl:id>GAZ:00128911</oboInOwl:id>
        <rdfs:label>Ryangdong-ri</rdfs:label>
    </owl:NamedIndividual>
    


    <!-- http://purl.obolibrary.org/obo/GAZ_00128912 -->

    <owl:NamedIndividual rdf:about="http://purl.obolibrary.org/obo/GAZ_00128912">
        <rdf:type rdf:resource="http://purl.obolibrary.org/obo/ENVO_00000856"/>
        <obo:RO_0001025 rdf:resource="http://purl.obolibrary.org/obo/GAZ_00027828"/>
        <obo:IAO_0000115>A populated place. A village of Saebyol County.</obo:IAO_0000115>
        <oboInOwl:hasOBONamespace>GAZ</oboInOwl:hasOBONamespace>
        <oboInOwl:id>GAZ:00128912</oboInOwl:id>
        <rdfs:label>Husok-ri</rdfs:label>
    </owl:NamedIndividual>
    


    <!-- http://purl.obolibrary.org/obo/GAZ_00128913 -->

    <owl:NamedIndividual rdf:about="http://purl.obolibrary.org/obo/GAZ_00128913">
        <rdf:type rdf:resource="http://purl.obolibrary.org/obo/ENVO_00000856"/>
        <obo:RO_0001025 rdf:resource="http://purl.obolibrary.org/obo/GAZ_00027819"/>
        <obo:IAO_0000115>A populated place. A town of Undok County.</obo:IAO_0000115>
        <oboInOwl:hasOBONamespace>GAZ</oboInOwl:hasOBONamespace>
        <oboInOwl:id>GAZ:00128913</oboInOwl:id>
        <rdfs:label>Undok-up</rdfs:label>
    </owl:NamedIndividual>
    


    <!-- http://purl.obolibrary.org/obo/GAZ_00128914 -->

    <owl:NamedIndividual rdf:about="http://purl.obolibrary.org/obo/GAZ_00128914">
        <obo:RO_0001025 rdf:resource="http://purl.obolibrary.org/obo/GAZ_00027819"/>
        <obo:IAO_0000115>A &apos;worker&apos;s district&apos; of Undok County.</obo:IAO_0000115>
        <oboInOwl:hasOBONamespace>GAZ</oboInOwl:hasOBONamespace>
        <oboInOwl:id>GAZ:00128914</oboInOwl:id>
        <rdfs:label>Obong-rodongjagu</rdfs:label>
    </owl:NamedIndividual>
    


    <!-- http://purl.obolibrary.org/obo/GAZ_00128915 -->

    <owl:NamedIndividual rdf:about="http://purl.obolibrary.org/obo/GAZ_00128915">
        <obo:RO_0001025 rdf:resource="http://purl.obolibrary.org/obo/GAZ_00027819"/>
        <obo:IAO_0000115>A &apos;worker&apos;s district&apos; of Undok County.</obo:IAO_0000115>
        <oboInOwl:hasOBONamespace>GAZ</oboInOwl:hasOBONamespace>
        <oboInOwl:id>GAZ:00128915</oboInOwl:id>
        <rdfs:label>Myongryong-rodongjagu</rdfs:label>
    </owl:NamedIndividual>
    


    <!-- http://purl.obolibrary.org/obo/GAZ_00128916 -->

    <owl:NamedIndividual rdf:about="http://purl.obolibrary.org/obo/GAZ_00128916">
        <obo:RO_0001025 rdf:resource="http://purl.obolibrary.org/obo/GAZ_00027819"/>
        <obo:IAO_0000115>A &apos;worker&apos;s district&apos; of Undok County.</obo:IAO_0000115>
        <oboInOwl:hasOBONamespace>GAZ</oboInOwl:hasOBONamespace>
        <oboInOwl:id>GAZ:00128916</oboInOwl:id>
        <rdfs:label>Ryongyon-rodongjagu</rdfs:label>
    </owl:NamedIndividual>
    


    <!-- http://purl.obolibrary.org/obo/GAZ_00128917 -->

    <owl:NamedIndividual rdf:about="http://purl.obolibrary.org/obo/GAZ_00128917">
        <rdf:type rdf:resource="http://purl.obolibrary.org/obo/ENVO_00000856"/>
        <obo:RO_0001025 rdf:resource="http://purl.obolibrary.org/obo/GAZ_00027819"/>
        <obo:IAO_0000115>A populated place. A village of Undok County.</obo:IAO_0000115>
        <oboInOwl:hasOBONamespace>GAZ</oboInOwl:hasOBONamespace>
        <oboInOwl:id>GAZ:00128917</oboInOwl:id>
        <rdfs:label>Rokya-ri</rdfs:label>
    </owl:NamedIndividual>
    


    <!-- http://purl.obolibrary.org/obo/GAZ_00128918 -->

    <owl:NamedIndividual rdf:about="http://purl.obolibrary.org/obo/GAZ_00128918">
        <rdf:type rdf:resource="http://purl.obolibrary.org/obo/ENVO_00000856"/>
        <obo:RO_0001025 rdf:resource="http://purl.obolibrary.org/obo/GAZ_00027819"/>
        <obo:IAO_0000115>A populated place. A village of Undok County.</obo:IAO_0000115>
        <oboInOwl:hasOBONamespace>GAZ</oboInOwl:hasOBONamespace>
        <oboInOwl:id>GAZ:00128918</oboInOwl:id>
        <rdfs:label>Taeyang-ri</rdfs:label>
    </owl:NamedIndividual>
    


    <!-- http://purl.obolibrary.org/obo/GAZ_00128919 -->

    <owl:NamedIndividual rdf:about="http://purl.obolibrary.org/obo/GAZ_00128919">
        <rdf:type rdf:resource="http://purl.obolibrary.org/obo/ENVO_00000856"/>
        <obo:RO_0001025 rdf:resource="http://purl.obolibrary.org/obo/GAZ_00027819"/>
        <obo:IAO_0000115>A populated place. A village of Undok County.</obo:IAO_0000115>
        <oboInOwl:hasOBONamespace>GAZ</oboInOwl:hasOBONamespace>
        <oboInOwl:id>GAZ:00128919</oboInOwl:id>
        <rdfs:label>Angil-ri</rdfs:label>
    </owl:NamedIndividual>
    


    <!-- http://purl.obolibrary.org/obo/GAZ_00128920 -->

    <owl:NamedIndividual rdf:about="http://purl.obolibrary.org/obo/GAZ_00128920">
        <rdf:type rdf:resource="http://purl.obolibrary.org/obo/ENVO_00000856"/>
        <obo:RO_0001025 rdf:resource="http://purl.obolibrary.org/obo/GAZ_00027819"/>
        <obo:IAO_0000115>A populated place. A village of Undok County.</obo:IAO_0000115>
        <oboInOwl:hasOBONamespace>GAZ</oboInOwl:hasOBONamespace>
        <oboInOwl:id>GAZ:00128920</oboInOwl:id>
        <rdfs:label>Cholchu-ri</rdfs:label>
    </owl:NamedIndividual>
    


    <!-- http://purl.obolibrary.org/obo/GAZ_00128921 -->

    <owl:NamedIndividual rdf:about="http://purl.obolibrary.org/obo/GAZ_00128921">
        <rdf:type rdf:resource="http://purl.obolibrary.org/obo/ENVO_00000856"/>
        <obo:RO_0001025 rdf:resource="http://purl.obolibrary.org/obo/GAZ_00027819"/>
        <obo:IAO_0000115>A populated place. A village of Undok County.</obo:IAO_0000115>
        <oboInOwl:hasOBONamespace>GAZ</oboInOwl:hasOBONamespace>
        <oboInOwl:id>GAZ:00128921</oboInOwl:id>
        <rdfs:label>Myongdok-ri</rdfs:label>
    </owl:NamedIndividual>
    


    <!-- http://purl.obolibrary.org/obo/GAZ_00128922 -->

    <owl:NamedIndividual rdf:about="http://purl.obolibrary.org/obo/GAZ_00128922">
        <rdf:type rdf:resource="http://purl.obolibrary.org/obo/ENVO_00000856"/>
        <obo:RO_0001025 rdf:resource="http://purl.obolibrary.org/obo/GAZ_00027819"/>
        <obo:IAO_0000115>A populated place. A village of Undok County.</obo:IAO_0000115>
        <oboInOwl:hasOBONamespace>GAZ</oboInOwl:hasOBONamespace>
        <oboInOwl:id>GAZ:00128922</oboInOwl:id>
        <rdfs:label>Songhak-ri</rdfs:label>
    </owl:NamedIndividual>
    


    <!-- http://purl.obolibrary.org/obo/GAZ_00128923 -->

    <owl:NamedIndividual rdf:about="http://purl.obolibrary.org/obo/GAZ_00128923">
        <rdf:type rdf:resource="http://purl.obolibrary.org/obo/ENVO_00000856"/>
        <obo:RO_0001025 rdf:resource="http://purl.obolibrary.org/obo/GAZ_00027819"/>
        <obo:IAO_0000115>A populated place. A village of Undok County.</obo:IAO_0000115>
        <oboInOwl:hasOBONamespace>GAZ</oboInOwl:hasOBONamespace>
        <oboInOwl:id>GAZ:00128923</oboInOwl:id>
        <rdfs:label>Kwirak-ri</rdfs:label>
    </owl:NamedIndividual>
    


    <!-- http://purl.obolibrary.org/obo/GAZ_00128924 -->

    <owl:NamedIndividual rdf:about="http://purl.obolibrary.org/obo/GAZ_00128924">
        <rdf:type rdf:resource="http://purl.obolibrary.org/obo/ENVO_00000856"/>
        <obo:RO_0001025 rdf:resource="http://purl.obolibrary.org/obo/GAZ_00027819"/>
        <obo:IAO_0000115>A populated place. A village of Undok County.</obo:IAO_0000115>
        <oboInOwl:hasOBONamespace>GAZ</oboInOwl:hasOBONamespace>
        <oboInOwl:id>GAZ:00128924</oboInOwl:id>
        <rdfs:label>Sinasan-ri</rdfs:label>
    </owl:NamedIndividual>
    


    <!-- http://purl.obolibrary.org/obo/GAZ_00128925 -->

    <owl:NamedIndividual rdf:about="http://purl.obolibrary.org/obo/GAZ_00128925">
        <rdf:type rdf:resource="http://purl.obolibrary.org/obo/ENVO_00000856"/>
        <obo:RO_0001025 rdf:resource="http://purl.obolibrary.org/obo/GAZ_00027819"/>
        <obo:IAO_0000115>A populated place. A village of Undok County.</obo:IAO_0000115>
        <oboInOwl:hasOBONamespace>GAZ</oboInOwl:hasOBONamespace>
        <oboInOwl:id>GAZ:00128925</oboInOwl:id>
        <rdfs:label>Haksong-ri</rdfs:label>
    </owl:NamedIndividual>
    


    <!-- http://purl.obolibrary.org/obo/GAZ_00128926 -->

    <owl:NamedIndividual rdf:about="http://purl.obolibrary.org/obo/GAZ_00128926">
        <rdf:type rdf:resource="http://purl.obolibrary.org/obo/ENVO_00000856"/>
        <obo:RO_0001025 rdf:resource="http://purl.obolibrary.org/obo/GAZ_00027819"/>
        <obo:IAO_0000115>A populated place. A village of Undok County.</obo:IAO_0000115>
        <oboInOwl:hasOBONamespace>GAZ</oboInOwl:hasOBONamespace>
        <oboInOwl:id>GAZ:00128926</oboInOwl:id>
        <rdfs:label>Changpyong-ri</rdfs:label>
    </owl:NamedIndividual>
    


    <!-- http://purl.obolibrary.org/obo/GAZ_00128927 -->

    <owl:NamedIndividual rdf:about="http://purl.obolibrary.org/obo/GAZ_00128927">
        <rdf:type rdf:resource="http://purl.obolibrary.org/obo/ENVO_00000856"/>
        <obo:RO_0001025 rdf:resource="http://purl.obolibrary.org/obo/GAZ_00027819"/>
        <obo:IAO_0000115>A populated place. A village of Undok County.</obo:IAO_0000115>
        <oboInOwl:hasOBONamespace>GAZ</oboInOwl:hasOBONamespace>
        <oboInOwl:id>GAZ:00128927</oboInOwl:id>
        <rdfs:label>Songsan-ri</rdfs:label>
    </owl:NamedIndividual>
    


    <!-- http://purl.obolibrary.org/obo/GAZ_00128928 -->

    <owl:NamedIndividual rdf:about="http://purl.obolibrary.org/obo/GAZ_00128928">
        <rdf:type rdf:resource="http://purl.obolibrary.org/obo/ENVO_00000856"/>
        <obo:RO_0001025 rdf:resource="http://purl.obolibrary.org/obo/GAZ_00027819"/>
        <obo:IAO_0000115>A populated place. A village of Undok County.</obo:IAO_0000115>
        <oboInOwl:hasOBONamespace>GAZ</oboInOwl:hasOBONamespace>
        <oboInOwl:id>GAZ:00128928</oboInOwl:id>
        <rdfs:label>Kumsong-ri</rdfs:label>
    </owl:NamedIndividual>
    


    <!-- http://purl.obolibrary.org/obo/GAZ_00128929 -->

    <owl:NamedIndividual rdf:about="http://purl.obolibrary.org/obo/GAZ_00128929">
        <obo:RO_0001025 rdf:resource="http://purl.obolibrary.org/obo/GAZ_00027802"/>
        <obo:IAO_0000115>An island.</obo:IAO_0000115>
        <oboInOwl:hasOBONamespace>GAZ</oboInOwl:hasOBONamespace>
        <oboInOwl:id>GAZ:00128929</oboInOwl:id>
        <rdfs:label>Choncho-do</rdfs:label>
    </owl:NamedIndividual>
    


    <!-- http://purl.obolibrary.org/obo/GAZ_00128930 -->

    <owl:NamedIndividual rdf:about="http://purl.obolibrary.org/obo/GAZ_00128930">
        <obo:RO_0001025 rdf:resource="http://purl.obolibrary.org/obo/GAZ_00027802"/>
        <obo:IAO_0000115>An island.</obo:IAO_0000115>
        <oboInOwl:hasOBONamespace>GAZ</oboInOwl:hasOBONamespace>
        <oboInOwl:id>GAZ:00128930</oboInOwl:id>
        <rdfs:label>Chintu-do</rdfs:label>
    </owl:NamedIndividual>
    


    <!-- http://purl.obolibrary.org/obo/GAZ_00128976 -->

    <owl:NamedIndividual rdf:about="http://purl.obolibrary.org/obo/GAZ_00128976">
        <obo:RO_0001025 rdf:resource="http://purl.obolibrary.org/obo/GAZ_00027816"/>
        <obo:IAO_0000115>Mountains.</obo:IAO_0000115>
        <oboInOwl:hasOBONamespace>GAZ</oboInOwl:hasOBONamespace>
        <oboInOwl:id>GAZ:00128976</oboInOwl:id>
        <rdfs:label>Taedok Mountains</rdfs:label>
    </owl:NamedIndividual>
    


    <!-- http://purl.obolibrary.org/obo/GAZ_00128977 -->

    <owl:NamedIndividual rdf:about="http://purl.obolibrary.org/obo/GAZ_00128977">
        <obo:RO_0001025 rdf:resource="http://purl.obolibrary.org/obo/GAZ_00027813"/>
        <obo:IAO_0000115>A reservoir.</obo:IAO_0000115>
        <oboInOwl:hasOBONamespace>GAZ</oboInOwl:hasOBONamespace>
        <oboInOwl:id>GAZ:00128977</oboInOwl:id>
        <rdfs:label>Lake Changjin</rdfs:label>
    </owl:NamedIndividual>
    


    <!-- http://purl.obolibrary.org/obo/GAZ_00128979 -->

    <owl:NamedIndividual rdf:about="http://purl.obolibrary.org/obo/GAZ_00128979">
        <obo:RO_0001025 rdf:resource="http://purl.obolibrary.org/obo/GAZ_02000761"/>
        <obo:IAO_0000115>A peninsula jutting out into the Yellow Sea. The Ongjin Peninsula is further divided into the Kangryong Peninsula, the Tongnam Peninsula, and the Ryongch&apos;on Peninsula. Geologically, Ongjin County is composed of coastal Lias. The Ongjin Plain, Kangryong Bay, Hwasan Bay, and Taedong Bay are all located here.</obo:IAO_0000115>
        <oboInOwl:hasOBONamespace>GAZ</oboInOwl:hasOBONamespace>
        <oboInOwl:id>GAZ:00128979</oboInOwl:id>
        <rdfs:label>Ongjin Peninsula</rdfs:label>
    </owl:NamedIndividual>
    


    <!-- http://purl.obolibrary.org/obo/GAZ_00128980 -->

    <owl:NamedIndividual rdf:about="http://purl.obolibrary.org/obo/GAZ_00128980">
        <obo:RO_0001025 rdf:resource="http://purl.obolibrary.org/obo/GAZ_00128979"/>
        <obo:IAO_0000115>A peninsula on the Ongjin Peninsula, North Korea.</obo:IAO_0000115>
        <oboInOwl:hasOBONamespace>GAZ</oboInOwl:hasOBONamespace>
        <oboInOwl:id>GAZ:00128980</oboInOwl:id>
        <rdfs:label>Kangryong Peninsula</rdfs:label>
    </owl:NamedIndividual>
    


    <!-- http://purl.obolibrary.org/obo/GAZ_00128981 -->

    <owl:NamedIndividual rdf:about="http://purl.obolibrary.org/obo/GAZ_00128981">
        <obo:RO_0001025 rdf:resource="http://purl.obolibrary.org/obo/GAZ_00128979"/>
        <obo:IAO_0000115>A peninsula on the Ongjin Peninsula, North Korea.</obo:IAO_0000115>
        <oboInOwl:hasOBONamespace>GAZ</oboInOwl:hasOBONamespace>
        <oboInOwl:id>GAZ:00128981</oboInOwl:id>
        <rdfs:label>Ryongch&apos;on Peninsula</rdfs:label>
    </owl:NamedIndividual>
    


    <!-- http://purl.obolibrary.org/obo/GAZ_00128982 -->

    <owl:NamedIndividual rdf:about="http://purl.obolibrary.org/obo/GAZ_00128982">
        <obo:RO_0001025 rdf:resource="http://purl.obolibrary.org/obo/GAZ_00128979"/>
        <obo:IAO_0000115>A peninsula on the Ongjin Peninsula, North Korea.</obo:IAO_0000115>
        <oboInOwl:hasOBONamespace>GAZ</oboInOwl:hasOBONamespace>
        <oboInOwl:id>GAZ:00128982</oboInOwl:id>
        <rdfs:label>Tongnam Peninsula</rdfs:label>
    </owl:NamedIndividual>
    


    <!-- http://purl.obolibrary.org/obo/GAZ_00128986 -->

    <owl:NamedIndividual rdf:about="http://purl.obolibrary.org/obo/GAZ_00128986">
        <obo:RO_0001025 rdf:resource="http://purl.obolibrary.org/obo/GAZ_00027773"/>
        <obo:IAO_0000115>A mountain range.</obo:IAO_0000115>
        <oboInOwl:hasOBONamespace>GAZ</oboInOwl:hasOBONamespace>
        <oboInOwl:id>GAZ:00128986</oboInOwl:id>
        <rdfs:label>Pult&apos;a Mountains</rdfs:label>
    </owl:NamedIndividual>
    


    <!-- http://purl.obolibrary.org/obo/GAZ_00128987 -->

    <owl:NamedIndividual rdf:about="http://purl.obolibrary.org/obo/GAZ_00128987">
        <obo:RO_0001025 rdf:resource="http://purl.obolibrary.org/obo/GAZ_00128986"/>
        <obo:IAO_0000115>A projection of the Pult&apos;a Mountains into the Yellow Sea.</obo:IAO_0000115>
        <oboInOwl:hasOBONamespace>GAZ</oboInOwl:hasOBONamespace>
        <oboInOwl:id>GAZ:00128987</oboInOwl:id>
        <rdfs:label>Changsan Cape</rdfs:label>
    </owl:NamedIndividual>
    


    <!-- http://purl.obolibrary.org/obo/GAZ_00128988 -->

    <owl:NamedIndividual rdf:about="http://purl.obolibrary.org/obo/GAZ_00128988">
        <obo:RO_0001025 rdf:resource="http://purl.obolibrary.org/obo/GAZ_00128987"/>
        <obo:IAO_0000115>A sand dune; A National Mounument.</obo:IAO_0000115>
        <oboInOwl:hasOBONamespace>GAZ</oboInOwl:hasOBONamespace>
        <oboInOwl:id>GAZ:00128988</oboInOwl:id>
        <rdfs:label>Monggump&apos;o Sand Dune</rdfs:label>
    </owl:NamedIndividual>
    


    <!-- http://purl.obolibrary.org/obo/GAZ_00128989 -->

    <owl:NamedIndividual rdf:about="http://purl.obolibrary.org/obo/GAZ_00128989"/>
    


    <!-- http://purl.obolibrary.org/obo/GAZ_00128990 -->

    <owl:NamedIndividual rdf:about="http://purl.obolibrary.org/obo/GAZ_00128990"/>
    


    <!-- http://purl.obolibrary.org/obo/GAZ_00128991 -->

    <owl:NamedIndividual rdf:about="http://purl.obolibrary.org/obo/GAZ_00128991"/>
    


    <!-- http://purl.obolibrary.org/obo/GAZ_00128993 -->

    <owl:NamedIndividual rdf:about="http://purl.obolibrary.org/obo/GAZ_00128993">
        <obo:RO_0001025 rdf:resource="http://purl.obolibrary.org/obo/GAZ_00002801"/>
        <obo:RO_0001025 rdf:resource="http://purl.obolibrary.org/obo/GAZ_00027711"/>
        <obo:RO_0001025 rdf:resource="http://purl.obolibrary.org/obo/GAZ_00027746"/>
        <obo:RO_0001025 rdf:resource="http://purl.obolibrary.org/obo/GAZ_00027747"/>
        <obo:RO_0001025 rdf:resource="http://purl.obolibrary.org/obo/GAZ_00027748"/>
        <obo:IAO_0000115>A mountain range.</obo:IAO_0000115>
        <oboInOwl:hasOBONamespace>GAZ</oboInOwl:hasOBONamespace>
        <oboInOwl:id>GAZ:00128993</oboInOwl:id>
        <rdfs:label>Masikryong Mountains</rdfs:label>
    </owl:NamedIndividual>
    


    <!-- http://purl.obolibrary.org/obo/GAZ_00128994 -->

    <owl:NamedIndividual rdf:about="http://purl.obolibrary.org/obo/GAZ_00128994">
        <obo:RO_0001025 rdf:resource="http://purl.obolibrary.org/obo/GAZ_00002801"/>
        <obo:RO_0001025 rdf:resource="http://purl.obolibrary.org/obo/GAZ_00027748"/>
        <obo:IAO_0000115>A mountain range.</obo:IAO_0000115>
        <oboInOwl:hasOBONamespace>GAZ</oboInOwl:hasOBONamespace>
        <oboInOwl:id>GAZ:00128994</oboInOwl:id>
        <rdfs:label>Sokko Mountains</rdfs:label>
    </owl:NamedIndividual>
    


    <!-- http://purl.obolibrary.org/obo/GAZ_00128995 -->

    <owl:NamedIndividual rdf:about="http://purl.obolibrary.org/obo/GAZ_00128995">
        <obo:RO_0001025 rdf:resource="http://purl.obolibrary.org/obo/GAZ_00002801"/>
        <obo:RO_0001025 rdf:resource="http://purl.obolibrary.org/obo/GAZ_00027748"/>
        <obo:IAO_0000115>A mountain range.</obo:IAO_0000115>
        <oboInOwl:hasOBONamespace>GAZ</oboInOwl:hasOBONamespace>
        <oboInOwl:id>GAZ:00128995</oboInOwl:id>
        <rdfs:label>Ch&apos;onryong Mountains</rdfs:label>
    </owl:NamedIndividual>
    


    <!-- http://purl.obolibrary.org/obo/GAZ_00128996 -->

    <owl:NamedIndividual rdf:about="http://purl.obolibrary.org/obo/GAZ_00128996">
        <obo:RO_0001025 rdf:resource="http://purl.obolibrary.org/obo/GAZ_00027742"/>
        <obo:IAO_0000115>An island.</obo:IAO_0000115>
        <oboInOwl:hasOBONamespace>GAZ</oboInOwl:hasOBONamespace>
        <oboInOwl:id>GAZ:00128996</oboInOwl:id>
        <rdfs:label>Ryo Island</rdfs:label>
    </owl:NamedIndividual>
    


    <!-- http://purl.obolibrary.org/obo/GAZ_00128997 -->

    <owl:NamedIndividual rdf:about="http://purl.obolibrary.org/obo/GAZ_00128997">
        <obo:RO_0001025 rdf:resource="http://purl.obolibrary.org/obo/GAZ_00027742"/>
        <obo:IAO_0000115>An island.</obo:IAO_0000115>
        <oboInOwl:hasOBONamespace>GAZ</oboInOwl:hasOBONamespace>
        <oboInOwl:id>GAZ:00128997</oboInOwl:id>
        <rdfs:label>Hwangt&apos;o Island</rdfs:label>
    </owl:NamedIndividual>
    


    <!-- http://purl.obolibrary.org/obo/GAZ_00128998 -->

    <owl:NamedIndividual rdf:about="http://purl.obolibrary.org/obo/GAZ_00128998">
        <obo:RO_0001025 rdf:resource="http://purl.obolibrary.org/obo/GAZ_00027747"/>
        <obo:IAO_0000115>A mountain range.</obo:IAO_0000115>
        <oboInOwl:hasOBONamespace>GAZ</oboInOwl:hasOBONamespace>
        <oboInOwl:id>GAZ:00128998</oboInOwl:id>
        <rdfs:label>Ahobiryong Mountains</rdfs:label>
    </owl:NamedIndividual>
    


    <!-- http://purl.obolibrary.org/obo/GAZ_00128999 -->

    <owl:NamedIndividual rdf:about="http://purl.obolibrary.org/obo/GAZ_00128999">
        <obo:RO_0001025 rdf:resource="http://purl.obolibrary.org/obo/GAZ_00027752"/>
        <obo:RO_0001025 rdf:resource="http://purl.obolibrary.org/obo/GAZ_00027758"/>
        <obo:IAO_0000115>A wetland.</obo:IAO_0000115>
        <oboInOwl:hasOBONamespace>GAZ</oboInOwl:hasOBONamespace>
        <oboInOwl:id>GAZ:00128999</oboInOwl:id>
        <rdfs:label>Yongam Wetland</rdfs:label>
    </owl:NamedIndividual>
    


    <!-- http://purl.obolibrary.org/obo/GAZ_00129000 -->

    <owl:NamedIndividual rdf:about="http://purl.obolibrary.org/obo/GAZ_00129000">
        <obo:RO_0001025 rdf:resource="http://purl.obolibrary.org/obo/GAZ_00027724"/>
        <obo:RO_0001025 rdf:resource="http://purl.obolibrary.org/obo/GAZ_00027736"/>
        <obo:RO_0001025 rdf:resource="http://purl.obolibrary.org/obo/GAZ_00027739"/>
        <obo:IAO_0000115>A mountain range.</obo:IAO_0000115>
        <oboInOwl:hasOBONamespace>GAZ</oboInOwl:hasOBONamespace>
        <oboInOwl:id>GAZ:00129000</oboInOwl:id>
        <rdfs:label>Pinandok Mountains</rdfs:label>
    </owl:NamedIndividual>
    


    <!-- http://purl.obolibrary.org/obo/GAZ_00129001 -->

    <owl:NamedIndividual rdf:about="http://purl.obolibrary.org/obo/GAZ_00129001">
        <obo:RO_0001025 rdf:resource="http://purl.obolibrary.org/obo/GAZ_00027739"/>
        <obo:IAO_0000115>An artificial lake in Ch&apos;angsong County, North Korea caused by damming the Yalu River.</obo:IAO_0000115>
        <oboInOwl:hasOBONamespace>GAZ</oboInOwl:hasOBONamespace>
        <oboInOwl:id>GAZ:00129001</oboInOwl:id>
        <rdfs:label>Supung Lake</rdfs:label>
    </owl:NamedIndividual>
    


    <!-- http://purl.obolibrary.org/obo/GAZ_00129002 -->

    <owl:NamedIndividual rdf:about="http://purl.obolibrary.org/obo/GAZ_00129002">
        <rdf:type rdf:resource="http://purl.obolibrary.org/obo/ENVO_00000220"/>
        <obo:RO_0001025 rdf:resource="http://purl.obolibrary.org/obo/GAZ_00027718"/>
        <obo:RO_0001025 rdf:resource="http://purl.obolibrary.org/obo/GAZ_00027735"/>
        <obo:IAO_0000115>An island group.</obo:IAO_0000115>
        <oboInOwl:hasOBONamespace>GAZ</oboInOwl:hasOBONamespace>
        <oboInOwl:id>GAZ:00129002</oboInOwl:id>
        <rdfs:label>Pansong Archipelago</rdfs:label>
    </owl:NamedIndividual>
    


    <!-- http://purl.obolibrary.org/obo/GAZ_00129003 -->

    <owl:NamedIndividual rdf:about="http://purl.obolibrary.org/obo/GAZ_00129003">
        <obo:RO_0001025 rdf:resource="http://purl.obolibrary.org/obo/GAZ_00027718"/>
        <obo:IAO_0000115>An island.</obo:IAO_0000115>
        <oboInOwl:hasOBONamespace>GAZ</oboInOwl:hasOBONamespace>
        <oboInOwl:id>GAZ:00129003</oboInOwl:id>
        <rdfs:label>Won-do</rdfs:label>
    </owl:NamedIndividual>
    


    <!-- http://purl.obolibrary.org/obo/GAZ_00129004 -->

    <owl:NamedIndividual rdf:about="http://purl.obolibrary.org/obo/GAZ_00129004">
        <obo:RO_0001025 rdf:resource="http://purl.obolibrary.org/obo/GAZ_00027729"/>
        <obo:IAO_0000115>A reservoir.</obo:IAO_0000115>
        <oboInOwl:hasOBONamespace>GAZ</oboInOwl:hasOBONamespace>
        <oboInOwl:id>GAZ:00129004</oboInOwl:id>
        <rdfs:label>Taeha Reservoir</rdfs:label>
    </owl:NamedIndividual>
    


    <!-- http://purl.obolibrary.org/obo/GAZ_00129005 -->

    <owl:NamedIndividual rdf:about="http://purl.obolibrary.org/obo/GAZ_00129005">
        <obo:RO_0001025 rdf:resource="http://purl.obolibrary.org/obo/GAZ_00027729"/>
        <obo:IAO_0000115>An artificial lake.</obo:IAO_0000115>
        <oboInOwl:hasOBONamespace>GAZ</oboInOwl:hasOBONamespace>
        <oboInOwl:id>GAZ:00129005</oboInOwl:id>
        <rdfs:label>Manpung Lake</rdfs:label>
    </owl:NamedIndividual>
    


    <!-- http://purl.obolibrary.org/obo/GAZ_00129006 -->

    <owl:NamedIndividual rdf:about="http://purl.obolibrary.org/obo/GAZ_00129006">
        <obo:RO_0001025 rdf:resource="http://purl.obolibrary.org/obo/GAZ_00027722"/>
        <obo:IAO_0000115>A mountain range.</obo:IAO_0000115>
        <oboInOwl:hasOBONamespace>GAZ</oboInOwl:hasOBONamespace>
        <oboInOwl:id>GAZ:00129006</oboInOwl:id>
        <rdfs:label>Munsu Mountains</rdfs:label>
    </owl:NamedIndividual>
    


    <!-- http://purl.obolibrary.org/obo/GAZ_00129007 -->

    <owl:NamedIndividual rdf:about="http://purl.obolibrary.org/obo/GAZ_00129007">
        <obo:RO_0001025 rdf:resource="http://purl.obolibrary.org/obo/GAZ_00027728"/>
        <obo:RO_0001025 rdf:resource="http://purl.obolibrary.org/obo/GAZ_00129008"/>
        <obo:IAO_0000115>An island in the estuary of the Yalu River. It was formed by a 1958 reclamation project from several smaller islands.</obo:IAO_0000115>
        <oboInOwl:hasOBONamespace>GAZ</oboInOwl:hasOBONamespace>
        <oboInOwl:id>GAZ:00129007</oboInOwl:id>
        <rdfs:label>Pidansom</rdfs:label>
    </owl:NamedIndividual>
    


    <!-- http://purl.obolibrary.org/obo/GAZ_00129008 -->

    <owl:NamedIndividual rdf:about="http://purl.obolibrary.org/obo/GAZ_00129008">
        <obo:IAO_0000115>The estuary of the Yalu River.</obo:IAO_0000115>
        <oboInOwl:hasOBONamespace>GAZ</oboInOwl:hasOBONamespace>
        <oboInOwl:id>GAZ:00129008</oboInOwl:id>
        <rdfs:label>Yalu River estuary</rdfs:label>
    </owl:NamedIndividual>
    


    <!-- http://purl.obolibrary.org/obo/GAZ_00129009 -->

    <owl:NamedIndividual rdf:about="http://purl.obolibrary.org/obo/GAZ_00129009">
        <obo:RO_0001025 rdf:resource="http://purl.obolibrary.org/obo/GAZ_00027728"/>
        <obo:RO_0001025 rdf:resource="http://purl.obolibrary.org/obo/GAZ_00129008"/>
        <obo:IAO_0000115>An island in the estuary of the Yalu River.</obo:IAO_0000115>
        <oboInOwl:hasOBONamespace>GAZ</oboInOwl:hasOBONamespace>
        <oboInOwl:id>GAZ:00129009</oboInOwl:id>
        <rdfs:label>Ssarisom</rdfs:label>
    </owl:NamedIndividual>
    


    <!-- http://purl.obolibrary.org/obo/GAZ_00129010 -->

    <owl:NamedIndividual rdf:about="http://purl.obolibrary.org/obo/GAZ_00129010">
        <obo:RO_0001025 rdf:resource="http://purl.obolibrary.org/obo/GAZ_00027728"/>
        <obo:RO_0001025 rdf:resource="http://purl.obolibrary.org/obo/GAZ_00129008"/>
        <obo:IAO_0000115>An island in the estuary of the Yalu River.</obo:IAO_0000115>
        <oboInOwl:hasOBONamespace>GAZ</oboInOwl:hasOBONamespace>
        <oboInOwl:id>GAZ:00129010</oboInOwl:id>
        <rdfs:label>Kanunsom</rdfs:label>
    </owl:NamedIndividual>
    


    <!-- http://purl.obolibrary.org/obo/GAZ_00129011 -->

    <owl:NamedIndividual rdf:about="http://purl.obolibrary.org/obo/GAZ_00129011">
        <obo:RO_0001025 rdf:resource="http://purl.obolibrary.org/obo/GAZ_00027728"/>
        <obo:RO_0001025 rdf:resource="http://purl.obolibrary.org/obo/GAZ_00129008"/>
        <obo:IAO_0000115>An island in the estuary of the Yalu River.</obo:IAO_0000115>
        <oboInOwl:hasOBONamespace>GAZ</oboInOwl:hasOBONamespace>
        <oboInOwl:id>GAZ:00129011</oboInOwl:id>
        <rdfs:label>Munbakto</rdfs:label>
    </owl:NamedIndividual>
    


    <!-- http://purl.obolibrary.org/obo/GAZ_00129012 -->

    <owl:NamedIndividual rdf:about="http://purl.obolibrary.org/obo/GAZ_00129012">
        <obo:RO_0001025 rdf:resource="http://purl.obolibrary.org/obo/GAZ_00027732"/>
        <obo:IAO_0000115>An island.</obo:IAO_0000115>
        <oboInOwl:hasOBONamespace>GAZ</oboInOwl:hasOBONamespace>
        <oboInOwl:id>GAZ:00129012</oboInOwl:id>
        <rdfs:label>Sinmi-do</rdfs:label>
    </owl:NamedIndividual>
    


    <!-- http://purl.obolibrary.org/obo/GAZ_00129013 -->

    <owl:NamedIndividual rdf:about="http://purl.obolibrary.org/obo/GAZ_00129013">
        <obo:RO_0001025 rdf:resource="http://purl.obolibrary.org/obo/GAZ_00027720"/>
        <obo:IAO_0000115>An island.</obo:IAO_0000115>
        <oboInOwl:hasOBONamespace>GAZ</oboInOwl:hasOBONamespace>
        <oboInOwl:id>GAZ:00129013</oboInOwl:id>
        <rdfs:label>Unmu-do</rdfs:label>
    </owl:NamedIndividual>
    


    <!-- http://purl.obolibrary.org/obo/GAZ_00129014 -->

    <owl:NamedIndividual rdf:about="http://purl.obolibrary.org/obo/GAZ_00129014">
        <obo:RO_0001025 rdf:resource="http://purl.obolibrary.org/obo/GAZ_00027720"/>
        <obo:IAO_0000115>An island.</obo:IAO_0000115>
        <oboInOwl:hasOBONamespace>GAZ</oboInOwl:hasOBONamespace>
        <oboInOwl:id>GAZ:00129014</oboInOwl:id>
        <rdfs:label>Hoesung-do</rdfs:label>
    </owl:NamedIndividual>
    


    <!-- http://purl.obolibrary.org/obo/GAZ_00129015 -->

    <owl:NamedIndividual rdf:about="http://purl.obolibrary.org/obo/GAZ_00129015">
        <obo:RO_0001025 rdf:resource="http://purl.obolibrary.org/obo/GAZ_00027735"/>
        <obo:IAO_0000115>An island.</obo:IAO_0000115>
        <oboInOwl:hasOBONamespace>GAZ</oboInOwl:hasOBONamespace>
        <oboInOwl:id>GAZ:00129015</oboInOwl:id>
        <rdfs:label>Taedasa-do</rdfs:label>
    </owl:NamedIndividual>
    


    <!-- http://purl.obolibrary.org/obo/GAZ_00129016 -->

    <owl:NamedIndividual rdf:about="http://purl.obolibrary.org/obo/GAZ_00129016">
        <obo:RO_0001025 rdf:resource="http://purl.obolibrary.org/obo/GAZ_00027735"/>
        <obo:IAO_0000115>An island.</obo:IAO_0000115>
        <oboInOwl:hasOBONamespace>GAZ</oboInOwl:hasOBONamespace>
        <oboInOwl:id>GAZ:00129016</oboInOwl:id>
        <rdfs:label>Chang-do</rdfs:label>
    </owl:NamedIndividual>
    


    <!-- http://purl.obolibrary.org/obo/GAZ_00129017 -->

    <owl:NamedIndividual rdf:about="http://purl.obolibrary.org/obo/GAZ_00129017">
        <obo:RO_0001025 rdf:resource="http://purl.obolibrary.org/obo/GAZ_02000765"/>
        <obo:IAO_0000115>A county of P&apos;yongan-nam Province. Prior to 2004, it was Chonrima kuyok, a district of northeastern Nampho directly-governed city.</obo:IAO_0000115>
        <oboInOwl:hasOBONamespace>GAZ</oboInOwl:hasOBONamespace>
        <oboInOwl:id>GAZ:00129017</oboInOwl:id>
        <rdfs:label>Chonrima County</rdfs:label>
    </owl:NamedIndividual>
    


    <!-- http://purl.obolibrary.org/obo/GAZ_00129018 -->

    <owl:NamedIndividual rdf:about="http://purl.obolibrary.org/obo/GAZ_00129018">
        <obo:RO_0001025 rdf:resource="http://purl.obolibrary.org/obo/GAZ_02000765"/>
        <obo:IAO_0000115>A county of P&apos;yongan-nam Province.</obo:IAO_0000115>
        <oboInOwl:hasOBONamespace>GAZ</oboInOwl:hasOBONamespace>
        <oboInOwl:id>GAZ:00129018</oboInOwl:id>
        <rdfs:label>Kangso County</rdfs:label>
    </owl:NamedIndividual>
    


    <!-- http://purl.obolibrary.org/obo/GAZ_00129019 -->

    <owl:NamedIndividual rdf:about="http://purl.obolibrary.org/obo/GAZ_00129019">
        <obo:RO_0001025 rdf:resource="http://purl.obolibrary.org/obo/GAZ_02000765"/>
        <obo:IAO_0000115>A county of P&apos;yongan-nam Province.</obo:IAO_0000115>
        <oboInOwl:hasOBONamespace>GAZ</oboInOwl:hasOBONamespace>
        <oboInOwl:id>GAZ:00129019</oboInOwl:id>
        <rdfs:label>Maengsan County</rdfs:label>
    </owl:NamedIndividual>
    


    <!-- http://purl.obolibrary.org/obo/GAZ_00129020 -->

    <owl:NamedIndividual rdf:about="http://purl.obolibrary.org/obo/GAZ_00129020">
        <obo:RO_0001025 rdf:resource="http://purl.obolibrary.org/obo/GAZ_00027707"/>
        <obo:RO_0001025 rdf:resource="http://purl.obolibrary.org/obo/GAZ_00027714"/>
        <obo:IAO_0000115>A mountain range.</obo:IAO_0000115>
        <oboInOwl:hasOBONamespace>GAZ</oboInOwl:hasOBONamespace>
        <oboInOwl:id>GAZ:00129020</oboInOwl:id>
        <rdfs:label>Puksubaek Mountains</rdfs:label>
    </owl:NamedIndividual>
    


    <!-- http://purl.obolibrary.org/obo/GAZ_00129021 -->

    <owl:NamedIndividual rdf:about="http://purl.obolibrary.org/obo/GAZ_00129021">
        <obo:RO_0001025 rdf:resource="http://purl.obolibrary.org/obo/GAZ_00002801"/>
        <obo:IAO_0000115>A mountain range.</obo:IAO_0000115>
        <oboInOwl:hasOBONamespace>GAZ</oboInOwl:hasOBONamespace>
        <oboInOwl:id>GAZ:00129021</oboInOwl:id>
        <rdfs:label>Huisaekbong Mountains</rdfs:label>
    </owl:NamedIndividual>
    


    <!-- http://purl.obolibrary.org/obo/GAZ_00129022 -->

    <owl:NamedIndividual rdf:about="http://purl.obolibrary.org/obo/GAZ_00129022">
        <obo:RO_0001025 rdf:resource="http://purl.obolibrary.org/obo/GAZ_00027710"/>
        <obo:IAO_0000115>Three lakes.</obo:IAO_0000115>
        <oboInOwl:hasOBONamespace>GAZ</oboInOwl:hasOBONamespace>
        <oboInOwl:id>GAZ:00129022</oboInOwl:id>
        <rdfs:label>Samjiyon Lakes</rdfs:label>
    </owl:NamedIndividual>
    


    <!-- http://purl.obolibrary.org/obo/GAZ_00129023 -->

    <owl:NamedIndividual rdf:about="http://purl.obolibrary.org/obo/GAZ_00129023">
        <obo:RO_0001025 rdf:resource="http://purl.obolibrary.org/obo/GAZ_00010089"/>
        <oboInOwl:hasOBONamespace>GAZ</oboInOwl:hasOBONamespace>
        <oboInOwl:id>GAZ:00129023</oboInOwl:id>
        <rdfs:label>Pyongyang</rdfs:label>
    </owl:NamedIndividual>
    


    <!-- http://purl.obolibrary.org/obo/GAZ_00129024 -->

    <owl:NamedIndividual rdf:about="http://purl.obolibrary.org/obo/GAZ_00129024">
        <rdf:type rdf:resource="http://purl.obolibrary.org/obo/ENVO_00000856"/>
        <obo:RO_0001025 rdf:resource="http://purl.obolibrary.org/obo/GAZ_00027637"/>
        <obo:RO_0001025 rdf:resource="http://purl.obolibrary.org/obo/GAZ_00027718"/>
        <obo:IAO_0000115>A populated place. A village in Ch&apos;olsan County. Partly in the Sinuiju Special Administrative Region.</obo:IAO_0000115>
        <oboInOwl:hasOBONamespace>GAZ</oboInOwl:hasOBONamespace>
        <oboInOwl:id>GAZ:00129024</oboInOwl:id>
        <rdfs:label>Kumsan-ri</rdfs:label>
    </owl:NamedIndividual>
    


    <!-- http://purl.obolibrary.org/obo/GAZ_00129025 -->

    <owl:NamedIndividual rdf:about="http://purl.obolibrary.org/obo/GAZ_00129025">
        <rdf:type rdf:resource="http://purl.obolibrary.org/obo/ENVO_00000856"/>
        <obo:RO_0001025 rdf:resource="http://purl.obolibrary.org/obo/GAZ_00027637"/>
        <obo:RO_0001025 rdf:resource="http://purl.obolibrary.org/obo/GAZ_00027718"/>
        <obo:IAO_0000115>A populated place. A village in Ch&apos;olsan County. Partly in the Sinuiju Special Administrative Region.</obo:IAO_0000115>
        <oboInOwl:hasOBONamespace>GAZ</oboInOwl:hasOBONamespace>
        <oboInOwl:id>GAZ:00129025</oboInOwl:id>
        <rdfs:label>Rihwa-ri</rdfs:label>
    </owl:NamedIndividual>
    


    <!-- http://purl.obolibrary.org/obo/GAZ_00129026 -->

    <owl:NamedIndividual rdf:about="http://purl.obolibrary.org/obo/GAZ_00129026">
        <rdf:type rdf:resource="http://purl.obolibrary.org/obo/ENVO_00000856"/>
        <obo:RO_0001025 rdf:resource="http://purl.obolibrary.org/obo/GAZ_00027637"/>
        <obo:RO_0001025 rdf:resource="http://purl.obolibrary.org/obo/GAZ_00027639"/>
        <obo:IAO_0000115>A populated place. A village of Uiji County. Partly in the Sinuiju Special Administrative Region.</obo:IAO_0000115>
        <oboInOwl:hasOBONamespace>GAZ</oboInOwl:hasOBONamespace>
        <oboInOwl:id>GAZ:00129026</oboInOwl:id>
        <rdfs:label>Hongnam-ri</rdfs:label>
    </owl:NamedIndividual>
    


    <!-- http://purl.obolibrary.org/obo/GAZ_00129027 -->

    <owl:NamedIndividual rdf:about="http://purl.obolibrary.org/obo/GAZ_00129027">
        <rdf:type rdf:resource="http://purl.obolibrary.org/obo/ENVO_00000856"/>
        <obo:RO_0001025 rdf:resource="http://purl.obolibrary.org/obo/GAZ_00027637"/>
        <obo:RO_0001025 rdf:resource="http://purl.obolibrary.org/obo/GAZ_00027639"/>
        <obo:IAO_0000115>A populated place. A village of Uiji County. Partly in the Sinuiju Special Administrative Region.</obo:IAO_0000115>
        <oboInOwl:hasOBONamespace>GAZ</oboInOwl:hasOBONamespace>
        <oboInOwl:id>GAZ:00129027</oboInOwl:id>
        <rdfs:label>Taesan-ri</rdfs:label>
    </owl:NamedIndividual>
    


    <!-- http://purl.obolibrary.org/obo/GAZ_00129028 -->

    <owl:NamedIndividual rdf:about="http://purl.obolibrary.org/obo/GAZ_00129028">
        <rdf:type rdf:resource="http://purl.obolibrary.org/obo/ENVO_00000856"/>
        <obo:RO_0001025 rdf:resource="http://purl.obolibrary.org/obo/GAZ_00027637"/>
        <obo:RO_0001025 rdf:resource="http://purl.obolibrary.org/obo/GAZ_00027639"/>
        <obo:IAO_0000115>A populated place. A village of Uiji County. In the Sinuiju Special Administrative Region.</obo:IAO_0000115>
        <oboInOwl:hasOBONamespace>GAZ</oboInOwl:hasOBONamespace>
        <oboInOwl:id>GAZ:00129028</oboInOwl:id>
        <rdfs:label>Soho-ri</rdfs:label>
    </owl:NamedIndividual>
    


    <!-- http://purl.obolibrary.org/obo/GAZ_00129029 -->

    <owl:NamedIndividual rdf:about="http://purl.obolibrary.org/obo/GAZ_00129029">
        <rdf:type rdf:resource="http://purl.obolibrary.org/obo/ENVO_00000856"/>
        <obo:RO_0001025 rdf:resource="http://purl.obolibrary.org/obo/GAZ_00027637"/>
        <obo:RO_0001025 rdf:resource="http://purl.obolibrary.org/obo/GAZ_00027735"/>
        <obo:IAO_0000115>A populated place. A village of Yomju District. Partly in the Sinuiju Special Administrative Region.</obo:IAO_0000115>
        <oboInOwl:hasOBONamespace>GAZ</oboInOwl:hasOBONamespace>
        <oboInOwl:id>GAZ:00129029</oboInOwl:id>
        <rdfs:label>Sokam-ri</rdfs:label>
    </owl:NamedIndividual>
    


    <!-- http://purl.obolibrary.org/obo/GAZ_00129030 -->

    <owl:NamedIndividual rdf:about="http://purl.obolibrary.org/obo/GAZ_00129030">
        <obo:RO_0001025 rdf:resource="http://purl.obolibrary.org/obo/GAZ_00027637"/>
        <obo:RO_0001025 rdf:resource="http://purl.obolibrary.org/obo/GAZ_00027735"/>
        <obo:IAO_0000115>A &apos;worker&apos;s district&apos; of Yomju County. In the Sinuiju Special Administrative Region.</obo:IAO_0000115>
        <oboInOwl:hasOBONamespace>GAZ</oboInOwl:hasOBONamespace>
        <oboInOwl:id>GAZ:00129030</oboInOwl:id>
        <rdfs:label>Tasa-rodongjagu</rdfs:label>
    </owl:NamedIndividual>
    


    <!-- http://purl.obolibrary.org/obo/GAZ_00129031 -->

    <owl:NamedIndividual rdf:about="http://purl.obolibrary.org/obo/GAZ_00129031">
        <obo:RO_0001025 rdf:resource="http://purl.obolibrary.org/obo/GAZ_00027727"/>
        <obo:IAO_0000115>A neighborhood of Sinuiju City. Part of the Sinuiju Special Administrative Region.</obo:IAO_0000115>
        <oboInOwl:hasOBONamespace>GAZ</oboInOwl:hasOBONamespace>
        <oboInOwl:id>GAZ:00129031</oboInOwl:id>
        <rdfs:label>Sinwon-dong</rdfs:label>
    </owl:NamedIndividual>
    


    <!-- http://purl.obolibrary.org/obo/GAZ_00129032 -->

    <owl:NamedIndividual rdf:about="http://purl.obolibrary.org/obo/GAZ_00129032">
        <obo:RO_0001025 rdf:resource="http://purl.obolibrary.org/obo/GAZ_00027727"/>
        <obo:IAO_0000115>A neighborhood of Sinuiju City. Part of the Sinuiju Special Administrative Region.</obo:IAO_0000115>
        <oboInOwl:hasOBONamespace>GAZ</oboInOwl:hasOBONamespace>
        <oboInOwl:id>GAZ:00129032</oboInOwl:id>
        <rdfs:label>Paekun-dong</rdfs:label>
    </owl:NamedIndividual>
    


    <!-- http://purl.obolibrary.org/obo/GAZ_00129033 -->

    <owl:NamedIndividual rdf:about="http://purl.obolibrary.org/obo/GAZ_00129033">
        <obo:RO_0001025 rdf:resource="http://purl.obolibrary.org/obo/GAZ_00027727"/>
        <obo:IAO_0000115>A neighborhood of Sinuiju City. Part of the Sinuiju Special Administrative Region.</obo:IAO_0000115>
        <oboInOwl:hasOBONamespace>GAZ</oboInOwl:hasOBONamespace>
        <oboInOwl:id>GAZ:00129033</oboInOwl:id>
        <rdfs:label>Namsang-dong</rdfs:label>
    </owl:NamedIndividual>
    


    <!-- http://purl.obolibrary.org/obo/GAZ_00129034 -->

    <owl:NamedIndividual rdf:about="http://purl.obolibrary.org/obo/GAZ_00129034">
        <obo:RO_0001025 rdf:resource="http://purl.obolibrary.org/obo/GAZ_00027727"/>
        <obo:IAO_0000115>A neighborhood of Sinuiju City. Part of the Sinuiju Special Administrative Region.</obo:IAO_0000115>
        <oboInOwl:hasOBONamespace>GAZ</oboInOwl:hasOBONamespace>
        <oboInOwl:id>GAZ:00129034</oboInOwl:id>
        <rdfs:label>Paeksa-dong</rdfs:label>
    </owl:NamedIndividual>
    


    <!-- http://purl.obolibrary.org/obo/GAZ_00129035 -->

    <owl:NamedIndividual rdf:about="http://purl.obolibrary.org/obo/GAZ_00129035">
        <obo:RO_0001025 rdf:resource="http://purl.obolibrary.org/obo/GAZ_00027727"/>
        <obo:IAO_0000115>A neighborhood of Sinuiju City. Part of the Sinuiju Special Administrative Region.</obo:IAO_0000115>
        <oboInOwl:hasOBONamespace>GAZ</oboInOwl:hasOBONamespace>
        <oboInOwl:id>GAZ:00129035</oboInOwl:id>
        <rdfs:label>Ch&apos;aeha-dong</rdfs:label>
    </owl:NamedIndividual>
    


    <!-- http://purl.obolibrary.org/obo/GAZ_00129036 -->

    <owl:NamedIndividual rdf:about="http://purl.obolibrary.org/obo/GAZ_00129036">
        <obo:RO_0001025 rdf:resource="http://purl.obolibrary.org/obo/GAZ_00027727"/>
        <obo:IAO_0000115>A neighborhood of Sinuiju City. Part of the Sinuiju Special Administrative Region.</obo:IAO_0000115>
        <oboInOwl:hasOBONamespace>GAZ</oboInOwl:hasOBONamespace>
        <oboInOwl:id>GAZ:00129036</oboInOwl:id>
        <rdfs:label>Oil-dong</rdfs:label>
    </owl:NamedIndividual>
    


    <!-- http://purl.obolibrary.org/obo/GAZ_00129037 -->

    <owl:NamedIndividual rdf:about="http://purl.obolibrary.org/obo/GAZ_00129037">
        <obo:RO_0001025 rdf:resource="http://purl.obolibrary.org/obo/GAZ_00027727"/>
        <obo:IAO_0000115>A neighborhood of Sinuiju City. Part of the Sinuiju Special Administrative Region.</obo:IAO_0000115>
        <oboInOwl:hasOBONamespace>GAZ</oboInOwl:hasOBONamespace>
        <oboInOwl:id>GAZ:00129037</oboInOwl:id>
        <rdfs:label>Namso-dong</rdfs:label>
    </owl:NamedIndividual>
    


    <!-- http://purl.obolibrary.org/obo/GAZ_00129038 -->

    <owl:NamedIndividual rdf:about="http://purl.obolibrary.org/obo/GAZ_00129038">
        <obo:RO_0001025 rdf:resource="http://purl.obolibrary.org/obo/GAZ_00027727"/>
        <obo:IAO_0000115>A neighborhood of Sinuiju City. Part of the Sinuiju Special Administrative Region.</obo:IAO_0000115>
        <oboInOwl:hasOBONamespace>GAZ</oboInOwl:hasOBONamespace>
        <oboInOwl:id>GAZ:00129038</oboInOwl:id>
        <rdfs:label>Kwanmun-dong</rdfs:label>
    </owl:NamedIndividual>
    


    <!-- http://purl.obolibrary.org/obo/GAZ_00129039 -->

    <owl:NamedIndividual rdf:about="http://purl.obolibrary.org/obo/GAZ_00129039">
        <obo:RO_0001025 rdf:resource="http://purl.obolibrary.org/obo/GAZ_00027727"/>
        <obo:IAO_0000115>A neighborhood of Sinuiju City. Part of the Sinuiju Special Administrative Region.</obo:IAO_0000115>
        <oboInOwl:hasOBONamespace>GAZ</oboInOwl:hasOBONamespace>
        <oboInOwl:id>GAZ:00129039</oboInOwl:id>
        <rdfs:label>Apkang-dong</rdfs:label>
    </owl:NamedIndividual>
    


    <!-- http://purl.obolibrary.org/obo/GAZ_00129040 -->

    <owl:NamedIndividual rdf:about="http://purl.obolibrary.org/obo/GAZ_00129040">
        <obo:RO_0001025 rdf:resource="http://purl.obolibrary.org/obo/GAZ_00027727"/>
        <obo:IAO_0000115>A neighborhood of Sinuiju City. Part of the Sinuiju Special Administrative Region.</obo:IAO_0000115>
        <oboInOwl:hasOBONamespace>GAZ</oboInOwl:hasOBONamespace>
        <oboInOwl:id>GAZ:00129040</oboInOwl:id>
        <rdfs:label>Ch&apos;ongsong-dong</rdfs:label>
    </owl:NamedIndividual>
    


    <!-- http://purl.obolibrary.org/obo/GAZ_00129041 -->

    <owl:NamedIndividual rdf:about="http://purl.obolibrary.org/obo/GAZ_00129041">
        <obo:RO_0001025 rdf:resource="http://purl.obolibrary.org/obo/GAZ_00027727"/>
        <obo:IAO_0000115>A neighborhood of Sinuiju City. Part of the Sinuiju Special Administrative Region.</obo:IAO_0000115>
        <oboInOwl:hasOBONamespace>GAZ</oboInOwl:hasOBONamespace>
        <oboInOwl:id>GAZ:00129041</oboInOwl:id>
        <rdfs:label>Yokchon-dong</rdfs:label>
    </owl:NamedIndividual>
    


    <!-- http://purl.obolibrary.org/obo/GAZ_00129042 -->

    <owl:NamedIndividual rdf:about="http://purl.obolibrary.org/obo/GAZ_00129042">
        <obo:RO_0001025 rdf:resource="http://purl.obolibrary.org/obo/GAZ_00027727"/>
        <obo:IAO_0000115>A neighborhood of Sinuiju City. Part of the Sinuiju Special Administrative Region.</obo:IAO_0000115>
        <oboInOwl:hasOBONamespace>GAZ</oboInOwl:hasOBONamespace>
        <oboInOwl:id>GAZ:00129042</oboInOwl:id>
        <rdfs:label>Ponbu-dong</rdfs:label>
    </owl:NamedIndividual>
    


    <!-- http://purl.obolibrary.org/obo/GAZ_00129043 -->

    <owl:NamedIndividual rdf:about="http://purl.obolibrary.org/obo/GAZ_00129043">
        <obo:RO_0001025 rdf:resource="http://purl.obolibrary.org/obo/GAZ_00027727"/>
        <obo:IAO_0000115>A neighborhood of Sinuiju City. Part of the Sinuiju Special Administrative Region.</obo:IAO_0000115>
        <oboInOwl:hasOBONamespace>GAZ</oboInOwl:hasOBONamespace>
        <oboInOwl:id>GAZ:00129043</oboInOwl:id>
        <rdfs:label>Kunhwa-dong</rdfs:label>
    </owl:NamedIndividual>
    


    <!-- http://purl.obolibrary.org/obo/GAZ_00129044 -->

    <owl:NamedIndividual rdf:about="http://purl.obolibrary.org/obo/GAZ_00129044">
        <obo:RO_0001025 rdf:resource="http://purl.obolibrary.org/obo/GAZ_00027727"/>
        <obo:IAO_0000115>A neighborhood of Sinuiju City. Part of the Sinuiju Special Administrative Region.</obo:IAO_0000115>
        <oboInOwl:hasOBONamespace>GAZ</oboInOwl:hasOBONamespace>
        <oboInOwl:id>GAZ:00129044</oboInOwl:id>
        <rdfs:label>Namjung-dong</rdfs:label>
    </owl:NamedIndividual>
    


    <!-- http://purl.obolibrary.org/obo/GAZ_00129045 -->

    <owl:NamedIndividual rdf:about="http://purl.obolibrary.org/obo/GAZ_00129045">
        <obo:RO_0001025 rdf:resource="http://purl.obolibrary.org/obo/GAZ_00027727"/>
        <obo:IAO_0000115>A neighborhood of Sinuiju City. Part of the Sinuiju Special Administrative Region.</obo:IAO_0000115>
        <oboInOwl:hasOBONamespace>GAZ</oboInOwl:hasOBONamespace>
        <oboInOwl:id>GAZ:00129045</oboInOwl:id>
        <rdfs:label>Namha-dong</rdfs:label>
    </owl:NamedIndividual>
    


    <!-- http://purl.obolibrary.org/obo/GAZ_00129046 -->

    <owl:NamedIndividual rdf:about="http://purl.obolibrary.org/obo/GAZ_00129046">
        <obo:RO_0001025 rdf:resource="http://purl.obolibrary.org/obo/GAZ_00027727"/>
        <obo:IAO_0000115>A neighborhood of Sinuiju City. Part of the Sinuiju Special Administrative Region.</obo:IAO_0000115>
        <oboInOwl:hasOBONamespace>GAZ</oboInOwl:hasOBONamespace>
        <oboInOwl:id>GAZ:00129046</oboInOwl:id>
        <rdfs:label>Haebang-dong</rdfs:label>
    </owl:NamedIndividual>
    


    <!-- http://purl.obolibrary.org/obo/GAZ_00129047 -->

    <owl:NamedIndividual rdf:about="http://purl.obolibrary.org/obo/GAZ_00129047">
        <obo:RO_0001025 rdf:resource="http://purl.obolibrary.org/obo/GAZ_00027727"/>
        <obo:IAO_0000115>A neighborhood of Sinuiju City. Part of the Sinuiju Special Administrative Region.</obo:IAO_0000115>
        <oboInOwl:hasOBONamespace>GAZ</oboInOwl:hasOBONamespace>
        <oboInOwl:id>GAZ:00129047</oboInOwl:id>
        <rdfs:label>Nammin-dong</rdfs:label>
    </owl:NamedIndividual>
    


    <!-- http://purl.obolibrary.org/obo/GAZ_00129048 -->

    <owl:NamedIndividual rdf:about="http://purl.obolibrary.org/obo/GAZ_00129048">
        <obo:RO_0001025 rdf:resource="http://purl.obolibrary.org/obo/GAZ_00027727"/>
        <obo:IAO_0000115>A neighborhood of Sinuiju City. Part of the Sinuiju Special Administrative Region.</obo:IAO_0000115>
        <oboInOwl:hasOBONamespace>GAZ</oboInOwl:hasOBONamespace>
        <oboInOwl:id>GAZ:00129048</oboInOwl:id>
        <rdfs:label>Sinp&apos;o-dong</rdfs:label>
    </owl:NamedIndividual>
    


    <!-- http://purl.obolibrary.org/obo/GAZ_00129049 -->

    <owl:NamedIndividual rdf:about="http://purl.obolibrary.org/obo/GAZ_00129049">
        <obo:RO_0001025 rdf:resource="http://purl.obolibrary.org/obo/GAZ_00027727"/>
        <obo:IAO_0000115>A neighborhood of Sinuiju City. Part of the Sinuiju Special Administrative Region.</obo:IAO_0000115>
        <oboInOwl:hasOBONamespace>GAZ</oboInOwl:hasOBONamespace>
        <oboInOwl:id>GAZ:00129049</oboInOwl:id>
        <rdfs:label>Tongha-dong</rdfs:label>
    </owl:NamedIndividual>
    


    <!-- http://purl.obolibrary.org/obo/GAZ_00129050 -->

    <owl:NamedIndividual rdf:about="http://purl.obolibrary.org/obo/GAZ_00129050">
        <obo:RO_0001025 rdf:resource="http://purl.obolibrary.org/obo/GAZ_00027727"/>
        <obo:IAO_0000115>A neighborhood of Sinuiju City. Part of the Sinuiju Special Administrative Region.</obo:IAO_0000115>
        <oboInOwl:hasOBONamespace>GAZ</oboInOwl:hasOBONamespace>
        <oboInOwl:id>GAZ:00129050</oboInOwl:id>
        <rdfs:label>Sinnam-dong</rdfs:label>
    </owl:NamedIndividual>
    


    <!-- http://purl.obolibrary.org/obo/GAZ_00129051 -->

    <owl:NamedIndividual rdf:about="http://purl.obolibrary.org/obo/GAZ_00129051">
        <obo:RO_0001025 rdf:resource="http://purl.obolibrary.org/obo/GAZ_00027727"/>
        <obo:IAO_0000115>A neighborhood of Sinuiju City. Part of the Sinuiju Special Administrative Region.</obo:IAO_0000115>
        <oboInOwl:hasOBONamespace>GAZ</oboInOwl:hasOBONamespace>
        <oboInOwl:id>GAZ:00129051</oboInOwl:id>
        <rdfs:label>P&apos;yonghwa-dong</rdfs:label>
    </owl:NamedIndividual>
    


    <!-- http://purl.obolibrary.org/obo/GAZ_00129052 -->

    <owl:NamedIndividual rdf:about="http://purl.obolibrary.org/obo/GAZ_00129052">
        <obo:RO_0001025 rdf:resource="http://purl.obolibrary.org/obo/GAZ_00027727"/>
        <obo:IAO_0000115>A neighborhood of Sinuiju City. Part of the Sinuiju Special Administrative Region.</obo:IAO_0000115>
        <oboInOwl:hasOBONamespace>GAZ</oboInOwl:hasOBONamespace>
        <oboInOwl:id>GAZ:00129052</oboInOwl:id>
        <rdfs:label>Minp&apos;o-dong</rdfs:label>
    </owl:NamedIndividual>
    


    <!-- http://purl.obolibrary.org/obo/GAZ_00129053 -->

    <owl:NamedIndividual rdf:about="http://purl.obolibrary.org/obo/GAZ_00129053">
        <obo:RO_0001025 rdf:resource="http://purl.obolibrary.org/obo/GAZ_00027727"/>
        <obo:IAO_0000115>A neighborhood of Sinuiju City. Part of the Sinuiju Special Administrative Region.</obo:IAO_0000115>
        <oboInOwl:hasOBONamespace>GAZ</oboInOwl:hasOBONamespace>
        <oboInOwl:id>GAZ:00129053</oboInOwl:id>
        <rdfs:label>Sumun-dong</rdfs:label>
    </owl:NamedIndividual>
    


    <!-- http://purl.obolibrary.org/obo/GAZ_00129054 -->

    <owl:NamedIndividual rdf:about="http://purl.obolibrary.org/obo/GAZ_00129054">
        <obo:RO_0001025 rdf:resource="http://purl.obolibrary.org/obo/GAZ_00027727"/>
        <obo:IAO_0000115>A neighborhood of Sinuiju City. Part of the Sinuiju Special Administrative Region.</obo:IAO_0000115>
        <oboInOwl:hasOBONamespace>GAZ</oboInOwl:hasOBONamespace>
        <oboInOwl:id>GAZ:00129054</oboInOwl:id>
        <rdfs:label>Kaehyok-dong</rdfs:label>
    </owl:NamedIndividual>
    


    <!-- http://purl.obolibrary.org/obo/GAZ_00129055 -->

    <owl:NamedIndividual rdf:about="http://purl.obolibrary.org/obo/GAZ_00129055">
        <obo:RO_0001025 rdf:resource="http://purl.obolibrary.org/obo/GAZ_00027727"/>
        <obo:IAO_0000115>A neighborhood of Sinuiju City. Part of the Sinuiju Special Administrative Region.</obo:IAO_0000115>
        <oboInOwl:hasOBONamespace>GAZ</oboInOwl:hasOBONamespace>
        <oboInOwl:id>GAZ:00129055</oboInOwl:id>
        <rdfs:label>Namsong-dong</rdfs:label>
    </owl:NamedIndividual>
    


    <!-- http://purl.obolibrary.org/obo/GAZ_00129056 -->

    <owl:NamedIndividual rdf:about="http://purl.obolibrary.org/obo/GAZ_00129056">
        <obo:RO_0001025 rdf:resource="http://purl.obolibrary.org/obo/GAZ_00027727"/>
        <obo:IAO_0000115>A neighborhood of Sinuiju City. Part of the Sinuiju Special Administrative Region.</obo:IAO_0000115>
        <oboInOwl:hasOBONamespace>GAZ</oboInOwl:hasOBONamespace>
        <oboInOwl:id>GAZ:00129056</oboInOwl:id>
        <rdfs:label>Tongjung-dong</rdfs:label>
    </owl:NamedIndividual>
    


    <!-- http://purl.obolibrary.org/obo/GAZ_00129057 -->

    <owl:NamedIndividual rdf:about="http://purl.obolibrary.org/obo/GAZ_00129057">
        <obo:RO_0001025 rdf:resource="http://purl.obolibrary.org/obo/GAZ_00027727"/>
        <obo:IAO_0000115>A neighborhood of Sinuiju City. Partly in the Sinuiju Special Administrative Region.</obo:IAO_0000115>
        <oboInOwl:hasOBONamespace>GAZ</oboInOwl:hasOBONamespace>
        <oboInOwl:id>GAZ:00129057</oboInOwl:id>
        <rdfs:label>Sonsang-dong</rdfs:label>
    </owl:NamedIndividual>
    


    <!-- http://purl.obolibrary.org/obo/GAZ_00129058 -->

    <owl:NamedIndividual rdf:about="http://purl.obolibrary.org/obo/GAZ_00129058">
        <rdf:type rdf:resource="http://purl.obolibrary.org/obo/ENVO_00000004"/>
        <obo:RO_0001025 rdf:resource="http://purl.obolibrary.org/obo/GAZ_00129065"/>
        <obo:IAO_0000115>An administrative division of Ryusang-dong.</obo:IAO_0000115>
        <oboInOwl:hasOBONamespace>GAZ</oboInOwl:hasOBONamespace>
        <oboInOwl:id>GAZ:00129058</oboInOwl:id>
        <rdfs:label>Ryusang 2-dong</rdfs:label>
    </owl:NamedIndividual>
    


    <!-- http://purl.obolibrary.org/obo/GAZ_00129059 -->

    <owl:NamedIndividual rdf:about="http://purl.obolibrary.org/obo/GAZ_00129059">
        <obo:RO_0001025 rdf:resource="http://purl.obolibrary.org/obo/GAZ_00027727"/>
        <obo:IAO_0000115>A neighborhood of Sinuiju City. Part of the Sinuiju Special Administrative Region.</obo:IAO_0000115>
        <oboInOwl:hasOBONamespace>GAZ</oboInOwl:hasOBONamespace>
        <oboInOwl:id>GAZ:00129059</oboInOwl:id>
        <rdfs:label>Majon-dong</rdfs:label>
    </owl:NamedIndividual>
    


    <!-- http://purl.obolibrary.org/obo/GAZ_00129060 -->

    <owl:NamedIndividual rdf:about="http://purl.obolibrary.org/obo/GAZ_00129060">
        <obo:RO_0001025 rdf:resource="http://purl.obolibrary.org/obo/GAZ_00027727"/>
        <obo:IAO_0000115>A neighborhood of Sinuiju City. Part of the Sinuiju Special Administrative Region.</obo:IAO_0000115>
        <oboInOwl:hasOBONamespace>GAZ</oboInOwl:hasOBONamespace>
        <oboInOwl:id>GAZ:00129060</oboInOwl:id>
        <rdfs:label>Ch&apos;inson-dong</rdfs:label>
    </owl:NamedIndividual>
    


    <!-- http://purl.obolibrary.org/obo/GAZ_00129061 -->

    <owl:NamedIndividual rdf:about="http://purl.obolibrary.org/obo/GAZ_00129061">
        <obo:RO_0001025 rdf:resource="http://purl.obolibrary.org/obo/GAZ_00027727"/>
        <obo:IAO_0000115>A neighborhood of Sinuiju City. Part of the Sinuiju Special Administrative Region.</obo:IAO_0000115>
        <oboInOwl:hasOBONamespace>GAZ</oboInOwl:hasOBONamespace>
        <oboInOwl:id>GAZ:00129061</oboInOwl:id>
        <rdfs:label>Pangjik-dong</rdfs:label>
    </owl:NamedIndividual>
    


    <!-- http://purl.obolibrary.org/obo/GAZ_00129062 -->

    <owl:NamedIndividual rdf:about="http://purl.obolibrary.org/obo/GAZ_00129062">
        <rdf:type rdf:resource="http://purl.obolibrary.org/obo/ENVO_00000004"/>
        <obo:RO_0001025 rdf:resource="http://purl.obolibrary.org/obo/GAZ_00129060"/>
        <obo:IAO_0000115>An administrative division of Ch&apos;inson-dong.</obo:IAO_0000115>
        <oboInOwl:hasOBONamespace>GAZ</oboInOwl:hasOBONamespace>
        <oboInOwl:id>GAZ:00129062</oboInOwl:id>
        <rdfs:label>Ch&apos;inson 1-dong</rdfs:label>
    </owl:NamedIndividual>
    


    <!-- http://purl.obolibrary.org/obo/GAZ_00129063 -->

    <owl:NamedIndividual rdf:about="http://purl.obolibrary.org/obo/GAZ_00129063">
        <rdf:type rdf:resource="http://purl.obolibrary.org/obo/ENVO_00000004"/>
        <obo:RO_0001025 rdf:resource="http://purl.obolibrary.org/obo/GAZ_00129060"/>
        <obo:IAO_0000115>An administrative division of Ch&apos;inson-dong.</obo:IAO_0000115>
        <oboInOwl:hasOBONamespace>GAZ</oboInOwl:hasOBONamespace>
        <oboInOwl:id>GAZ:00129063</oboInOwl:id>
        <rdfs:label>Ch&apos;inson 2-dong</rdfs:label>
    </owl:NamedIndividual>
    


    <!-- http://purl.obolibrary.org/obo/GAZ_00129064 -->

    <owl:NamedIndividual rdf:about="http://purl.obolibrary.org/obo/GAZ_00129064">
        <obo:RO_0001025 rdf:resource="http://purl.obolibrary.org/obo/GAZ_00027727"/>
        <obo:IAO_0000115>A neighborhood of Sinuiju City. Part of the Sinuiju Special Administrative Region.</obo:IAO_0000115>
        <oboInOwl:hasOBONamespace>GAZ</oboInOwl:hasOBONamespace>
        <oboInOwl:id>GAZ:00129064</oboInOwl:id>
        <rdfs:label>Tongsang-dong</rdfs:label>
    </owl:NamedIndividual>
    


    <!-- http://purl.obolibrary.org/obo/GAZ_00129065 -->

    <owl:NamedIndividual rdf:about="http://purl.obolibrary.org/obo/GAZ_00129065">
        <obo:RO_0001025 rdf:resource="http://purl.obolibrary.org/obo/GAZ_00027727"/>
        <obo:IAO_0000115>A neighborhood of Sinuiju City. Partly in the Sinuiju Special Administrative Region.</obo:IAO_0000115>
        <oboInOwl:hasOBONamespace>GAZ</oboInOwl:hasOBONamespace>
        <oboInOwl:id>GAZ:00129065</oboInOwl:id>
        <rdfs:label>Ryusang-dong</rdfs:label>
    </owl:NamedIndividual>
    


    <!-- http://purl.obolibrary.org/obo/GAZ_00129066 -->

    <owl:NamedIndividual rdf:about="http://purl.obolibrary.org/obo/GAZ_00129066">
        <obo:RO_0001025 rdf:resource="http://purl.obolibrary.org/obo/GAZ_00129065"/>
        <oboInOwl:hasOBONamespace>GAZ</oboInOwl:hasOBONamespace>
        <oboInOwl:id>GAZ:00129066</oboInOwl:id>
        <rdfs:label>Ryusang 1-dong</rdfs:label>
    </owl:NamedIndividual>
    


    <!-- http://purl.obolibrary.org/obo/GAZ_00129067 -->

    <owl:NamedIndividual rdf:about="http://purl.obolibrary.org/obo/GAZ_00129067">
        <obo:RO_0001025 rdf:resource="http://purl.obolibrary.org/obo/GAZ_00027727"/>
        <obo:IAO_0000115>A neighborhood of Sinuiju City. Partly in the Sinuiju Special Administrative Region.</obo:IAO_0000115>
        <oboInOwl:hasOBONamespace>GAZ</oboInOwl:hasOBONamespace>
        <oboInOwl:id>GAZ:00129067</oboInOwl:id>
        <rdfs:label>Yonha-dong</rdfs:label>
    </owl:NamedIndividual>
    


    <!-- http://purl.obolibrary.org/obo/GAZ_00129068 -->

    <owl:NamedIndividual rdf:about="http://purl.obolibrary.org/obo/GAZ_00129068">
        <obo:RO_0001025 rdf:resource="http://purl.obolibrary.org/obo/GAZ_00027727"/>
        <obo:IAO_0000115>A neighborhood of Sinuiju City. Partly in the Sinuiju Special Administrative Region.</obo:IAO_0000115>
        <oboInOwl:hasOBONamespace>GAZ</oboInOwl:hasOBONamespace>
        <oboInOwl:id>GAZ:00129068</oboInOwl:id>
        <rdfs:label>Songhan-dong</rdfs:label>
    </owl:NamedIndividual>
    


    <!-- http://purl.obolibrary.org/obo/GAZ_00129069 -->

    <owl:NamedIndividual rdf:about="http://purl.obolibrary.org/obo/GAZ_00129069">
        <obo:RO_0001025 rdf:resource="http://purl.obolibrary.org/obo/GAZ_00027727"/>
        <obo:IAO_0000115>A neighborhood of Sinuiju City. Partly in the Sinuiju Special Administrative Region.</obo:IAO_0000115>
        <oboInOwl:hasOBONamespace>GAZ</oboInOwl:hasOBONamespace>
        <oboInOwl:id>GAZ:00129069</oboInOwl:id>
        <rdfs:label>Paekt&apos;u-dong</rdfs:label>
    </owl:NamedIndividual>
    


    <!-- http://purl.obolibrary.org/obo/GAZ_00129070 -->

    <owl:NamedIndividual rdf:about="http://purl.obolibrary.org/obo/GAZ_00129070">
        <rdf:type rdf:resource="http://purl.obolibrary.org/obo/ENVO_00000856"/>
        <obo:RO_0001025 rdf:resource="http://purl.obolibrary.org/obo/GAZ_00027727"/>
        <obo:IAO_0000115>A populated place. A village of Sinuiju City. Partly in the Sinuiju Special Administrative Region.</obo:IAO_0000115>
        <oboInOwl:hasOBONamespace>GAZ</oboInOwl:hasOBONamespace>
        <oboInOwl:id>GAZ:00129070</oboInOwl:id>
        <rdfs:label>T&apos;osong-ri</rdfs:label>
    </owl:NamedIndividual>
    


    <!-- http://purl.obolibrary.org/obo/GAZ_00129071 -->

    <owl:NamedIndividual rdf:about="http://purl.obolibrary.org/obo/GAZ_00129071">
        <rdf:type rdf:resource="http://purl.obolibrary.org/obo/ENVO_00000856"/>
        <obo:RO_0001025 rdf:resource="http://purl.obolibrary.org/obo/GAZ_00027727"/>
        <obo:IAO_0000115>A populated place. A village of Sinuiju City. Part of the Sinuiju Special Administrative Region.</obo:IAO_0000115>
        <oboInOwl:hasOBONamespace>GAZ</oboInOwl:hasOBONamespace>
        <oboInOwl:id>GAZ:00129071</oboInOwl:id>
        <rdfs:label>Taji-ri</rdfs:label>
    </owl:NamedIndividual>
    


    <!-- http://purl.obolibrary.org/obo/GAZ_00129072 -->

    <owl:NamedIndividual rdf:about="http://purl.obolibrary.org/obo/GAZ_00129072">
        <rdf:type rdf:resource="http://purl.obolibrary.org/obo/ENVO_00000856"/>
        <obo:RO_0001025 rdf:resource="http://purl.obolibrary.org/obo/GAZ_00027727"/>
        <obo:IAO_0000115>A populated place. A village of Sinuiju City. Partly in the Sinuiju Special Administrative Region.</obo:IAO_0000115>
        <oboInOwl:hasOBONamespace>GAZ</oboInOwl:hasOBONamespace>
        <oboInOwl:id>GAZ:00129072</oboInOwl:id>
        <rdfs:label>Ryuch&apos;o-ri</rdfs:label>
    </owl:NamedIndividual>
    


    <!-- http://purl.obolibrary.org/obo/GAZ_00129073 -->

    <owl:NamedIndividual rdf:about="http://purl.obolibrary.org/obo/GAZ_00129073">
        <rdf:type rdf:resource="http://purl.obolibrary.org/obo/ENVO_00000856"/>
        <obo:RO_0001025 rdf:resource="http://purl.obolibrary.org/obo/GAZ_00027727"/>
        <obo:IAO_0000115>A populated place. A village of Sinuiju City. Part of the Sinuiju Special Administrative Region.</obo:IAO_0000115>
        <oboInOwl:hasOBONamespace>GAZ</oboInOwl:hasOBONamespace>
        <oboInOwl:id>GAZ:00129073</oboInOwl:id>
        <rdfs:label>Hadan-ri</rdfs:label>
    </owl:NamedIndividual>
    


    <!-- http://purl.obolibrary.org/obo/GAZ_00129074 -->

    <owl:NamedIndividual rdf:about="http://purl.obolibrary.org/obo/GAZ_00129074">
        <rdf:type rdf:resource="http://purl.obolibrary.org/obo/ENVO_00000856"/>
        <obo:RO_0001025 rdf:resource="http://purl.obolibrary.org/obo/GAZ_00027727"/>
        <obo:IAO_0000115>A populated place. A village of Sinuiju City. Part of the Sinuiju Special Administrative Region.</obo:IAO_0000115>
        <oboInOwl:hasOBONamespace>GAZ</oboInOwl:hasOBONamespace>
        <oboInOwl:id>GAZ:00129074</oboInOwl:id>
        <rdfs:label>Sangdan-ri</rdfs:label>
    </owl:NamedIndividual>
    


    <!-- http://purl.obolibrary.org/obo/GAZ_00247362 -->

    <owl:NamedIndividual rdf:about="http://purl.obolibrary.org/obo/GAZ_00247362">
        <obo:IAO_0000115>A reservoir. Located on the Korean border 70 km northeast of Dandong, Liaoning Province.</obo:IAO_0000115>
        <oboInOwl:hasOBONamespace>GAZ</oboInOwl:hasOBONamespace>
        <oboInOwl:id>GAZ:00247362</oboInOwl:id>
        <rdfs:label>Shuifeng Reservoir</rdfs:label>
    </owl:NamedIndividual>
    


    <!-- http://purl.obolibrary.org/obo/GAZ_00247606 -->

    <owl:NamedIndividual rdf:about="http://purl.obolibrary.org/obo/GAZ_00247606">
        <rdf:type rdf:resource="http://purl.obolibrary.org/obo/ENVO_00000029"/>
        <obo:RO_0001025 rdf:resource="http://purl.obolibrary.org/obo/GAZ_00054834"/>
        <obo:IAO_0000115>A branch of the Changbai Mountains on the China-North Korea border, start from eastern Jilin Province, China, and extend to eastern and southern Liaoning Province, down to Liaodong Peninsula.</obo:IAO_0000115>
        <oboInOwl:hasOBONamespace>GAZ</oboInOwl:hasOBONamespace>
        <oboInOwl:id>GAZ:00247606</oboInOwl:id>
        <rdfs:label>Qian Mountains</rdfs:label>
    </owl:NamedIndividual>
    


    <!-- http://purl.obolibrary.org/obo/GAZ_00251683 -->

    <owl:NamedIndividual rdf:about="http://purl.obolibrary.org/obo/GAZ_00251683">
        <obo:RO_0001025 rdf:resource="http://purl.obolibrary.org/obo/GAZ_00129022"/>
        <obo:IAO_0000115>A natural freshwater lake. Located in a region of old ash fields at the lowest point in the valley between Mount Paekdu to the north and another volcanic vent (Bukpotee) to the south.</obo:IAO_0000115>
        <oboInOwl:hasOBONamespace>GAZ</oboInOwl:hasOBONamespace>
        <oboInOwl:id>GAZ:00251683</oboInOwl:id>
        <rdfs:label>Lake Samjiyon</rdfs:label>
    </owl:NamedIndividual>
    


    <!-- http://purl.obolibrary.org/obo/GAZ_00251684 -->

    <owl:NamedIndividual rdf:about="http://purl.obolibrary.org/obo/GAZ_00251684">
        <obo:RO_0001025 rdf:resource="http://purl.obolibrary.org/obo/GAZ_00027686"/>
        <obo:IAO_0000115>A wetland. An area of marshes and peat bogs up to seven metres deep in the Hamgyong-Sanmaek Mountains.</obo:IAO_0000115>
        <oboInOwl:hasOBONamespace>GAZ</oboInOwl:hasOBONamespace>
        <oboInOwl:id>GAZ:00251684</oboInOwl:id>
        <rdfs:label>Kanjan-Nup Swamp</rdfs:label>
    </owl:NamedIndividual>
    


    <!-- http://purl.obolibrary.org/obo/GAZ_00251685 -->

    <owl:NamedIndividual rdf:about="http://purl.obolibrary.org/obo/GAZ_00251685">
        <obo:RO_0001025 rdf:resource="http://purl.obolibrary.org/obo/GAZ_00027686"/>
        <obo:RO_0001025 rdf:resource="http://purl.obolibrary.org/obo/GAZ_00027823"/>
        <obo:RO_0001025 rdf:resource="http://purl.obolibrary.org/obo/GAZ_00128847"/>
        <obo:IAO_0000115>A water storage reservoir on a tributary of the Tumen River. The reservoir is situated in forested hills near the Chinese border, at the north end of the Hamgyong-Sanmaek Mountains.</obo:IAO_0000115>
        <oboInOwl:hasOBONamespace>GAZ</oboInOwl:hasOBONamespace>
        <oboInOwl:id>GAZ:00251685</oboInOwl:id>
        <rdfs:label>Mayang Chosuji</rdfs:label>
    </owl:NamedIndividual>
    


    <!-- http://purl.obolibrary.org/obo/GAZ_00251687 -->

    <owl:NamedIndividual rdf:about="http://purl.obolibrary.org/obo/GAZ_00251687">
        <obo:RO_0001025 rdf:resource="http://purl.obolibrary.org/obo/GAZ_02000763"/>
        <obo:IAO_0000115>A populated place. A city in northern part of North Korea, and northern portion of the North Hamgyong Province. It lies on the Tumen River and opposite to the city of Tumen that stands in the Chinese bank of the river.</obo:IAO_0000115>
        <oboInOwl:hasOBONamespace>GAZ</oboInOwl:hasOBONamespace>
        <oboInOwl:id>GAZ:00251687</oboInOwl:id>
        <rdfs:label>Namyang</rdfs:label>
    </owl:NamedIndividual>
    


    <!-- http://purl.obolibrary.org/obo/GAZ_00251688 -->

    <owl:NamedIndividual rdf:about="http://purl.obolibrary.org/obo/GAZ_00251688">
        <obo:IAO_0000115>The delta of the Tumen River.</obo:IAO_0000115>
        <oboInOwl:hasOBONamespace>GAZ</oboInOwl:hasOBONamespace>
        <oboInOwl:id>GAZ:00251688</oboInOwl:id>
        <rdfs:label>Tumen Delta</rdfs:label>
    </owl:NamedIndividual>
    


    <!-- http://purl.obolibrary.org/obo/GAZ_00251689 -->

    <owl:NamedIndividual rdf:about="http://purl.obolibrary.org/obo/GAZ_00251689">
        <obo:RO_0001025 rdf:resource="http://purl.obolibrary.org/obo/GAZ_00251688"/>
        <obo:IAO_0000115>Three fresh/brackish lakes. Located on the border with Russia, 10-20 km east of Unggi and 90 km northeast of Chongjin, North Hamgyong Province.</obo:IAO_0000115>
        <oboInOwl:hasOBONamespace>GAZ</oboInOwl:hasOBONamespace>
        <oboInOwl:id>GAZ:00251689</oboInOwl:id>
        <rdfs:label>Unggi Lakes</rdfs:label>
    </owl:NamedIndividual>
    


    <!-- http://purl.obolibrary.org/obo/GAZ_00251690 -->

    <owl:NamedIndividual rdf:about="http://purl.obolibrary.org/obo/GAZ_00251690">
        <rdf:type rdf:resource="http://purl.obolibrary.org/obo/ENVO_00000856"/>
        <obo:RO_0001025 rdf:resource="http://purl.obolibrary.org/obo/GAZ_00027817"/>
        <obo:IAO_0000115>A populated place. A village.</obo:IAO_0000115>
        <oboInOwl:hasOBONamespace>GAZ</oboInOwl:hasOBONamespace>
        <oboInOwl:id>GAZ:00251690</oboInOwl:id>
        <rdfs:label>Ryon Pyon-ri</rdfs:label>
    </owl:NamedIndividual>
    


    <!-- http://purl.obolibrary.org/obo/GAZ_00251692 -->

    <owl:NamedIndividual rdf:about="http://purl.obolibrary.org/obo/GAZ_00251692">
        <obo:RO_0001025 rdf:resource="http://purl.obolibrary.org/obo/GAZ_00027807"/>
        <obo:IAO_0000115>A brackish lake. Formed by the natural damming of an estuarine system; the largest inland sea-lake in Korea. The lake is fed by the Wonsuchon and Pupyorchon Rivers, which rise in the hills to the west. Located 10 km south of Hungnam City, Chongpyong County, South Hamgyong Province.</obo:IAO_0000115>
        <oboInOwl:hasOBONamespace>GAZ</oboInOwl:hasOBONamespace>
        <oboInOwl:id>GAZ:00251692</oboInOwl:id>
        <rdfs:label>Kwan-Po</rdfs:label>
    </owl:NamedIndividual>
    


    <!-- http://purl.obolibrary.org/obo/GAZ_00251693 -->

    <owl:NamedIndividual rdf:about="http://purl.obolibrary.org/obo/GAZ_00251693">
        <obo:RO_0001025 rdf:resource="http://purl.obolibrary.org/obo/GAZ_00251692"/>
        <obo:IAO_0000115>A river.</obo:IAO_0000115>
        <oboInOwl:hasOBONamespace>GAZ</oboInOwl:hasOBONamespace>
        <oboInOwl:id>GAZ:00251693</oboInOwl:id>
        <rdfs:label>Wonsuchon River</rdfs:label>
    </owl:NamedIndividual>
    


    <!-- http://purl.obolibrary.org/obo/GAZ_00251694 -->

    <owl:NamedIndividual rdf:about="http://purl.obolibrary.org/obo/GAZ_00251694">
        <obo:RO_0001025 rdf:resource="http://purl.obolibrary.org/obo/GAZ_00251692"/>
        <obo:IAO_0000115>A river.</obo:IAO_0000115>
        <oboInOwl:hasOBONamespace>GAZ</oboInOwl:hasOBONamespace>
        <oboInOwl:id>GAZ:00251694</oboInOwl:id>
        <rdfs:label>Pupyorchon River</rdfs:label>
    </owl:NamedIndividual>
    


    <!-- http://purl.obolibrary.org/obo/GAZ_00251695 -->

    <owl:NamedIndividual rdf:about="http://purl.obolibrary.org/obo/GAZ_00251695">
        <rdf:type rdf:resource="http://purl.obolibrary.org/obo/ENVO_00000856"/>
        <obo:RO_0001025 rdf:resource="http://purl.obolibrary.org/obo/GAZ_00027754"/>
        <obo:IAO_0000115>A populated place. A village.</obo:IAO_0000115>
        <oboInOwl:hasOBONamespace>GAZ</oboInOwl:hasOBONamespace>
        <oboInOwl:id>GAZ:00251695</oboInOwl:id>
        <rdfs:label>Kanwon-ri</rdfs:label>
    </owl:NamedIndividual>
    


    <!-- http://purl.obolibrary.org/obo/GAZ_00251696 -->

    <owl:NamedIndividual rdf:about="http://purl.obolibrary.org/obo/GAZ_00251696">
        <obo:RO_0001025 rdf:resource="http://purl.obolibrary.org/obo/GAZ_00251695"/>
        <obo:IAO_0000115>A saline lake.</obo:IAO_0000115>
        <oboInOwl:hasOBONamespace>GAZ</oboInOwl:hasOBONamespace>
        <oboInOwl:id>GAZ:00251696</oboInOwl:id>
        <rdfs:label>Shijun-Ho</rdfs:label>
    </owl:NamedIndividual>
    


    <!-- http://purl.obolibrary.org/obo/GAZ_00251697 -->

    <owl:NamedIndividual rdf:about="http://purl.obolibrary.org/obo/GAZ_00251697">
        <rdf:type rdf:resource="http://purl.obolibrary.org/obo/ENVO_00000856"/>
        <obo:RO_0001025 rdf:resource="http://purl.obolibrary.org/obo/GAZ_00027750"/>
        <obo:IAO_0000115>A populated place. A village.</obo:IAO_0000115>
        <oboInOwl:hasOBONamespace>GAZ</oboInOwl:hasOBONamespace>
        <oboInOwl:id>GAZ:00251697</oboInOwl:id>
        <rdfs:label>Samil-Po-ri</rdfs:label>
    </owl:NamedIndividual>
    


    <!-- http://purl.obolibrary.org/obo/GAZ_00251698 -->

    <owl:NamedIndividual rdf:about="http://purl.obolibrary.org/obo/GAZ_00251698">
        <obo:RO_0001025 rdf:resource="http://purl.obolibrary.org/obo/GAZ_00251697"/>
        <obo:IAO_0000115>A freshwater lake.</obo:IAO_0000115>
        <oboInOwl:hasOBONamespace>GAZ</oboInOwl:hasOBONamespace>
        <oboInOwl:id>GAZ:00251698</oboInOwl:id>
        <rdfs:label>Samil-Po</rdfs:label>
    </owl:NamedIndividual>
    


    <!-- http://purl.obolibrary.org/obo/GAZ_00251700 -->

    <owl:NamedIndividual rdf:about="http://purl.obolibrary.org/obo/GAZ_00251700">
        <rdf:type rdf:resource="http://purl.obolibrary.org/obo/ENVO_00000856"/>
        <obo:RO_0001025 rdf:resource="http://purl.obolibrary.org/obo/GAZ_00027682"/>
        <obo:IAO_0000115>A populated place. A village.</obo:IAO_0000115>
        <oboInOwl:hasOBONamespace>GAZ</oboInOwl:hasOBONamespace>
        <oboInOwl:id>GAZ:00251700</oboInOwl:id>
        <rdfs:label>Tongrim-ri</rdfs:label>
    </owl:NamedIndividual>
    


    <!-- http://purl.obolibrary.org/obo/GAZ_00251702 -->

    <owl:NamedIndividual rdf:about="http://purl.obolibrary.org/obo/GAZ_00251702">
        <obo:RO_0001025 rdf:resource="http://purl.obolibrary.org/obo/GAZ_00251700"/>
        <obo:IAO_0000115>The estuary of the Chongchon-Gang River.</obo:IAO_0000115>
        <oboInOwl:hasOBONamespace>GAZ</oboInOwl:hasOBONamespace>
        <oboInOwl:id>GAZ:00251702</oboInOwl:id>
        <rdfs:label>Chongchon-Gang Estuary</rdfs:label>
    </owl:NamedIndividual>
    


    <!-- http://purl.obolibrary.org/obo/GAZ_00251703 -->

    <owl:NamedIndividual rdf:about="http://purl.obolibrary.org/obo/GAZ_00251703">
        <obo:RO_0001025 rdf:resource="http://purl.obolibrary.org/obo/GAZ_02000759"/>
        <obo:IAO_0000115>A small rocky island in the northeastern part of Korea Bay.</obo:IAO_0000115>
        <oboInOwl:hasOBONamespace>GAZ</oboInOwl:hasOBONamespace>
        <oboInOwl:id>GAZ:00251703</oboInOwl:id>
        <rdfs:label>Sogam-do</rdfs:label>
    </owl:NamedIndividual>
    


    <!-- http://purl.obolibrary.org/obo/GAZ_00251704 -->

    <owl:NamedIndividual rdf:about="http://purl.obolibrary.org/obo/GAZ_00251704">
        <obo:RO_0001025 rdf:resource="http://purl.obolibrary.org/obo/GAZ_02000759"/>
        <obo:IAO_0000115>A small rocky islands in the northeastern part of Korea Bay.</obo:IAO_0000115>
        <oboInOwl:hasOBONamespace>GAZ</oboInOwl:hasOBONamespace>
        <oboInOwl:id>GAZ:00251704</oboInOwl:id>
        <rdfs:label>Tegam-do</rdfs:label>
    </owl:NamedIndividual>
    


    <!-- http://purl.obolibrary.org/obo/GAZ_00251705 -->

    <owl:NamedIndividual rdf:about="http://purl.obolibrary.org/obo/GAZ_00251705">
        <obo:RO_0001025 rdf:resource="http://purl.obolibrary.org/obo/GAZ_02000759"/>
        <obo:IAO_0000115>Two small rocky islands in the northeastern part of Korea Bay.</obo:IAO_0000115>
        <oboInOwl:hasOBONamespace>GAZ</oboInOwl:hasOBONamespace>
        <oboInOwl:id>GAZ:00251705</oboInOwl:id>
        <rdfs:label>Sonchonrap-to</rdfs:label>
    </owl:NamedIndividual>
    


    <!-- http://purl.obolibrary.org/obo/GAZ_00251706 -->

    <owl:NamedIndividual rdf:about="http://purl.obolibrary.org/obo/GAZ_00251706">
        <obo:RO_0001025 rdf:resource="http://purl.obolibrary.org/obo/GAZ_00251705"/>
        <obo:IAO_0000115>A small rocky island in the northeastern part of Korea Bay.</obo:IAO_0000115>
        <oboInOwl:hasOBONamespace>GAZ</oboInOwl:hasOBONamespace>
        <oboInOwl:id>GAZ:00251706</oboInOwl:id>
        <rdfs:label>Rap-to</rdfs:label>
    </owl:NamedIndividual>
    


    <!-- http://purl.obolibrary.org/obo/GAZ_00251707 -->

    <owl:NamedIndividual rdf:about="http://purl.obolibrary.org/obo/GAZ_00251707">
        <obo:RO_0001025 rdf:resource="http://purl.obolibrary.org/obo/GAZ_00251705"/>
        <obo:IAO_0000115>A small rocky islands in the northeastern part of Korea Bay.</obo:IAO_0000115>
        <oboInOwl:hasOBONamespace>GAZ</oboInOwl:hasOBONamespace>
        <oboInOwl:id>GAZ:00251707</oboInOwl:id>
        <rdfs:label>Sorap-to</rdfs:label>
    </owl:NamedIndividual>
    


    <!-- http://purl.obolibrary.org/obo/GAZ_00251709 -->

    <owl:NamedIndividual rdf:about="http://purl.obolibrary.org/obo/GAZ_00251709">
        <obo:RO_0001025 rdf:resource="http://purl.obolibrary.org/obo/GAZ_02000756"/>
        <obo:IAO_0000115>A ward of Namp&apos;o Special City.</obo:IAO_0000115>
        <oboInOwl:hasOBONamespace>GAZ</oboInOwl:hasOBONamespace>
        <oboInOwl:id>GAZ:00251709</oboInOwl:id>
        <rdfs:label>Waudo-guyok</rdfs:label>
    </owl:NamedIndividual>
    


    <!-- http://purl.obolibrary.org/obo/GAZ_00251710 -->

    <owl:NamedIndividual rdf:about="http://purl.obolibrary.org/obo/GAZ_00251710">
        <obo:RO_0001025 rdf:resource="http://purl.obolibrary.org/obo/GAZ_02000756"/>
        <obo:IAO_0000115>A ward of Namp&apos;o Special City.</obo:IAO_0000115>
        <oboInOwl:hasOBONamespace>GAZ</oboInOwl:hasOBONamespace>
        <oboInOwl:id>GAZ:00251710</oboInOwl:id>
        <rdfs:label>Hanggu-guyok</rdfs:label>
    </owl:NamedIndividual>
    


    <!-- http://purl.obolibrary.org/obo/GAZ_00251711 -->

    <owl:NamedIndividual rdf:about="http://purl.obolibrary.org/obo/GAZ_00251711">
        <obo:RO_0001025 rdf:resource="http://purl.obolibrary.org/obo/GAZ_02000756"/>
        <obo:IAO_0000115>A county of Namp&apos;o Special City.</obo:IAO_0000115>
        <oboInOwl:hasOBONamespace>GAZ</oboInOwl:hasOBONamespace>
        <oboInOwl:id>GAZ:00251711</oboInOwl:id>
        <rdfs:label>Ch&apos;ollima-kun</rdfs:label>
    </owl:NamedIndividual>
    


    <!-- http://purl.obolibrary.org/obo/GAZ_00251712 -->

    <owl:NamedIndividual rdf:about="http://purl.obolibrary.org/obo/GAZ_00251712">
        <obo:RO_0001025 rdf:resource="http://purl.obolibrary.org/obo/GAZ_02000756"/>
        <obo:IAO_0000115>A county of Namp&apos;o Special City.</obo:IAO_0000115>
        <oboInOwl:hasOBONamespace>GAZ</oboInOwl:hasOBONamespace>
        <oboInOwl:id>GAZ:00251712</oboInOwl:id>
        <rdfs:label>Kangso-kun</rdfs:label>
    </owl:NamedIndividual>
    


    <!-- http://purl.obolibrary.org/obo/GAZ_00251713 -->

    <owl:NamedIndividual rdf:about="http://purl.obolibrary.org/obo/GAZ_00251713">
        <obo:RO_0001025 rdf:resource="http://purl.obolibrary.org/obo/GAZ_02000756"/>
        <obo:IAO_0000115>A county of Namp&apos;o Special City.</obo:IAO_0000115>
        <oboInOwl:hasOBONamespace>GAZ</oboInOwl:hasOBONamespace>
        <oboInOwl:id>GAZ:00251713</oboInOwl:id>
        <rdfs:label>Ryonggang-kun</rdfs:label>
    </owl:NamedIndividual>
    


    <!-- http://purl.obolibrary.org/obo/GAZ_00251714 -->

    <owl:NamedIndividual rdf:about="http://purl.obolibrary.org/obo/GAZ_00251714">
        <obo:RO_0001025 rdf:resource="http://purl.obolibrary.org/obo/GAZ_02000756"/>
        <obo:IAO_0000115>A county of Namp&apos;o Special City.</obo:IAO_0000115>
        <oboInOwl:hasOBONamespace>GAZ</oboInOwl:hasOBONamespace>
        <oboInOwl:id>GAZ:00251714</oboInOwl:id>
        <rdfs:label>Taean-kun</rdfs:label>
    </owl:NamedIndividual>
    


    <!-- http://purl.obolibrary.org/obo/GAZ_00251715 -->

    <owl:NamedIndividual rdf:about="http://purl.obolibrary.org/obo/GAZ_00251715">
        <rdf:type rdf:resource="http://purl.obolibrary.org/obo/ENVO_00000074"/>
        <obo:RO_0001025 rdf:resource="http://purl.obolibrary.org/obo/GAZ_02000756"/>
        <obo:IAO_0000115>A barrage located 15 km west of the special city of Nampho, North Korea. It is a huge, eight-km-long system of dams, three lock chambers, and 36 sluices, allowing the passage of ships up to 50,000 tons. The dam closes the Taedong River off from the Yellow Sea. Constructed 1981-1986.</obo:IAO_0000115>
        <oboInOwl:hasOBONamespace>GAZ</oboInOwl:hasOBONamespace>
        <oboInOwl:id>GAZ:00251715</oboInOwl:id>
        <rdfs:label>Nampho Dam</rdfs:label>
    </owl:NamedIndividual>
    


    <!-- http://purl.obolibrary.org/obo/GAZ_00251716 -->

    <owl:NamedIndividual rdf:about="http://purl.obolibrary.org/obo/GAZ_00251716">
        <obo:RO_0001025 rdf:resource="http://purl.obolibrary.org/obo/GAZ_02000756"/>
        <obo:IAO_0000115>A freshwater lake. It is located on the west bank of the Taedong River.</obo:IAO_0000115>
        <oboInOwl:hasOBONamespace>GAZ</oboInOwl:hasOBONamespace>
        <oboInOwl:id>GAZ:00251716</oboInOwl:id>
        <rdfs:label>Taesong-Ho</rdfs:label>
    </owl:NamedIndividual>
    


    <!-- http://purl.obolibrary.org/obo/GAZ_00251717 -->

    <owl:NamedIndividual rdf:about="http://purl.obolibrary.org/obo/GAZ_00251717">
        <obo:RO_0001025 rdf:resource="http://purl.obolibrary.org/obo/GAZ_02000766"/>
        <obo:IAO_0000115>An island. Off the estuary of the Taedong River.</obo:IAO_0000115>
        <oboInOwl:hasOBONamespace>GAZ</oboInOwl:hasOBONamespace>
        <oboInOwl:id>GAZ:00251717</oboInOwl:id>
        <rdfs:label>Tok-to</rdfs:label>
    </owl:NamedIndividual>
    


    <!-- http://purl.obolibrary.org/obo/GAZ_00251750 -->

    <owl:NamedIndividual rdf:about="http://purl.obolibrary.org/obo/GAZ_00251750">
        <obo:IAO_0000115>A resevoir.</obo:IAO_0000115>
        <oboInOwl:hasOBONamespace>GAZ</oboInOwl:hasOBONamespace>
        <oboInOwl:id>GAZ:00251750</oboInOwl:id>
        <rdfs:label>Andong Lake</rdfs:label>
    </owl:NamedIndividual>
    


    <!-- http://purl.obolibrary.org/obo/GAZ_00251751 -->

    <owl:NamedIndividual rdf:about="http://purl.obolibrary.org/obo/GAZ_00251751">
        <obo:IAO_0000115>Aa river in Mungyeong City, North Gyeongsang province, South Korea. It flows into the Nakdong River. The river rises from Hwabuk-myeon in Sangju, and drains most of western Mungyeong and parts of northern Sangju. The Yeong flows into the Nakdong at the southeastern corner of Mungyeong between Yeongsun-myeon and Sangju&apos;s Sabeol-myeon.</obo:IAO_0000115>
        <oboInOwl:hasOBONamespace>GAZ</oboInOwl:hasOBONamespace>
        <oboInOwl:id>GAZ:00251751</oboInOwl:id>
        <rdfs:label>Yeong River</rdfs:label>
    </owl:NamedIndividual>
    


    <!-- http://purl.obolibrary.org/obo/GAZ_00251754 -->

    <owl:NamedIndividual rdf:about="http://purl.obolibrary.org/obo/GAZ_00251754">
        <obo:IAO_0000115>The estuary of the Nakdong River. Located W of the citu of Busan.</obo:IAO_0000115>
        <oboInOwl:hasOBONamespace>GAZ</oboInOwl:hasOBONamespace>
        <oboInOwl:id>GAZ:00251754</oboInOwl:id>
        <rdfs:label>Nakdong Estuary</rdfs:label>
    </owl:NamedIndividual>
    


    <!-- http://purl.obolibrary.org/obo/GAZ_00251755 -->

    <owl:NamedIndividual rdf:about="http://purl.obolibrary.org/obo/GAZ_00251755">
        <obo:RO_0001025 rdf:resource="http://purl.obolibrary.org/obo/GAZ_00251754"/>
        <obo:IAO_0000115>An estuarine island.</obo:IAO_0000115>
        <oboInOwl:hasOBONamespace>GAZ</oboInOwl:hasOBONamespace>
        <oboInOwl:id>GAZ:00251755</oboInOwl:id>
        <rdfs:label>Galmaegi Deung</rdfs:label>
    </owl:NamedIndividual>
    


    <!-- http://purl.obolibrary.org/obo/GAZ_00251756 -->

    <owl:NamedIndividual rdf:about="http://purl.obolibrary.org/obo/GAZ_00251756">
        <obo:RO_0001025 rdf:resource="http://purl.obolibrary.org/obo/GAZ_00251754"/>
        <obo:IAO_0000115>An estuarine island.</obo:IAO_0000115>
        <oboInOwl:hasOBONamespace>GAZ</oboInOwl:hasOBONamespace>
        <oboInOwl:id>GAZ:00251756</oboInOwl:id>
        <rdfs:label>Namusit Deung</rdfs:label>
    </owl:NamedIndividual>
    


    <!-- http://purl.obolibrary.org/obo/GAZ_00251757 -->

    <owl:NamedIndividual rdf:about="http://purl.obolibrary.org/obo/GAZ_00251757">
        <obo:RO_0001025 rdf:resource="http://purl.obolibrary.org/obo/GAZ_00251754"/>
        <obo:IAO_0000115>An estuarine island.</obo:IAO_0000115>
        <oboInOwl:hasOBONamespace>GAZ</oboInOwl:hasOBONamespace>
        <oboInOwl:id>GAZ:00251757</oboInOwl:id>
        <rdfs:label>Jinuh do</rdfs:label>
    </owl:NamedIndividual>
    


    <!-- http://purl.obolibrary.org/obo/GAZ_00251758 -->

    <owl:NamedIndividual rdf:about="http://purl.obolibrary.org/obo/GAZ_00251758">
        <obo:RO_0001025 rdf:resource="http://purl.obolibrary.org/obo/GAZ_00251754"/>
        <obo:IAO_0000115>An estuarine island.</obo:IAO_0000115>
        <oboInOwl:hasOBONamespace>GAZ</oboInOwl:hasOBONamespace>
        <oboInOwl:id>GAZ:00251758</oboInOwl:id>
        <rdfs:label>Daema Deung</rdfs:label>
    </owl:NamedIndividual>
    


    <!-- http://purl.obolibrary.org/obo/GAZ_00251759 -->

    <owl:NamedIndividual rdf:about="http://purl.obolibrary.org/obo/GAZ_00251759">
        <obo:RO_0001025 rdf:resource="http://purl.obolibrary.org/obo/GAZ_00251754"/>
        <obo:IAO_0000115>An estuarine island.</obo:IAO_0000115>
        <oboInOwl:hasOBONamespace>GAZ</oboInOwl:hasOBONamespace>
        <oboInOwl:id>GAZ:00251759</oboInOwl:id>
        <rdfs:label>Ogryu Deung</rdfs:label>
    </owl:NamedIndividual>
    


    <!-- http://purl.obolibrary.org/obo/GAZ_00251760 -->

    <owl:NamedIndividual rdf:about="http://purl.obolibrary.org/obo/GAZ_00251760">
        <obo:RO_0001025 rdf:resource="http://purl.obolibrary.org/obo/GAZ_00251754"/>
        <obo:IAO_0000115>An estuarine island.</obo:IAO_0000115>
        <oboInOwl:hasOBONamespace>GAZ</oboInOwl:hasOBONamespace>
        <oboInOwl:id>GAZ:00251760</oboInOwl:id>
        <rdfs:label>Baeghab</rdfs:label>
    </owl:NamedIndividual>
    


    <!-- http://purl.obolibrary.org/obo/GAZ_00251761 -->

    <owl:NamedIndividual rdf:about="http://purl.obolibrary.org/obo/GAZ_00251761">
        <obo:RO_0001025 rdf:resource="http://purl.obolibrary.org/obo/GAZ_00251754"/>
        <obo:IAO_0000115>An estuarine island.</obo:IAO_0000115>
        <oboInOwl:hasOBONamespace>GAZ</oboInOwl:hasOBONamespace>
        <oboInOwl:id>GAZ:00251761</oboInOwl:id>
        <rdfs:label>Eulsuk do</rdfs:label>
    </owl:NamedIndividual>
    


    <!-- http://purl.obolibrary.org/obo/GAZ_00251762 -->

    <owl:NamedIndividual rdf:about="http://purl.obolibrary.org/obo/GAZ_00251762">
        <obo:RO_0001025 rdf:resource="http://purl.obolibrary.org/obo/GAZ_00251754"/>
        <obo:IAO_0000115>The W distributary of the Nakdong River.</obo:IAO_0000115>
        <oboInOwl:hasOBONamespace>GAZ</oboInOwl:hasOBONamespace>
        <oboInOwl:id>GAZ:00251762</oboInOwl:id>
        <rdfs:label>Jukrim Channel</rdfs:label>
    </owl:NamedIndividual>
    


    <!-- http://purl.obolibrary.org/obo/GAZ_00251763 -->

    <owl:NamedIndividual rdf:about="http://purl.obolibrary.org/obo/GAZ_00251763">
        <obo:RO_0001025 rdf:resource="http://purl.obolibrary.org/obo/GAZ_00251762"/>
        <obo:IAO_0000115>A dam.</obo:IAO_0000115>
        <oboInOwl:hasOBONamespace>GAZ</oboInOwl:hasOBONamespace>
        <oboInOwl:id>GAZ:00251763</oboInOwl:id>
        <rdfs:label>Noksan Dam</rdfs:label>
    </owl:NamedIndividual>
    


    <!-- http://purl.obolibrary.org/obo/GAZ_00251764 -->

    <owl:NamedIndividual rdf:about="http://purl.obolibrary.org/obo/GAZ_00251764">
        <rdf:type rdf:resource="http://purl.obolibrary.org/obo/ENVO_00000074"/>
        <obo:RO_0001025 rdf:resource="http://purl.obolibrary.org/obo/GAZ_00251754"/>
        <obo:IAO_0000115>A barrage. Constructed 1987.</obo:IAO_0000115>
        <oboInOwl:hasOBONamespace>GAZ</oboInOwl:hasOBONamespace>
        <oboInOwl:id>GAZ:00251764</oboInOwl:id>
        <rdfs:label>Nakdong Barrage</rdfs:label>
    </owl:NamedIndividual>
    


    <!-- http://purl.obolibrary.org/obo/GAZ_02000756 -->

    <owl:NamedIndividual rdf:about="http://purl.obolibrary.org/obo/GAZ_02000756">
        <obo:RO_0001025 rdf:resource="http://purl.obolibrary.org/obo/GAZ_02000765"/>
        <obo:IAO_0000115>A special city in P&apos;yongan-nam Province. It was a provincial-level Directly Governed City (Chikhalsi) from 1980 to 2004, when it was designated a Special City and made a part of P&apos;yongan-nam. Namp&apos;o lies on the northern shore of the Taedong River, 15 km east of the river&apos;s mouth.</obo:IAO_0000115>
        <oboInOwl:hasOBONamespace>GAZ</oboInOwl:hasOBONamespace>
        <oboInOwl:id>GAZ:02000756</oboInOwl:id>
        <rdfs:label>Namp&apos;o Special City</rdfs:label>
    </owl:NamedIndividual>
    


    <!-- http://purl.obolibrary.org/obo/GAZ_02000758 -->

    <owl:NamedIndividual rdf:about="http://purl.obolibrary.org/obo/GAZ_02000758"/>
    


    <!-- http://purl.obolibrary.org/obo/GAZ_02000759 -->

    <owl:NamedIndividual rdf:about="http://purl.obolibrary.org/obo/GAZ_02000759"/>
    


    <!-- http://purl.obolibrary.org/obo/GAZ_02000760 -->

    <owl:NamedIndividual rdf:about="http://purl.obolibrary.org/obo/GAZ_02000760"/>
    


    <!-- http://purl.obolibrary.org/obo/GAZ_02000761 -->

    <owl:NamedIndividual rdf:about="http://purl.obolibrary.org/obo/GAZ_02000761"/>
    


    <!-- http://purl.obolibrary.org/obo/GAZ_02000762 -->

    <owl:NamedIndividual rdf:about="http://purl.obolibrary.org/obo/GAZ_02000762"/>
    


    <!-- http://purl.obolibrary.org/obo/GAZ_02000763 -->

    <owl:NamedIndividual rdf:about="http://purl.obolibrary.org/obo/GAZ_02000763"/>
    


    <!-- http://purl.obolibrary.org/obo/GAZ_02000764 -->

    <owl:NamedIndividual rdf:about="http://purl.obolibrary.org/obo/GAZ_02000764"/>
    


    <!-- http://purl.obolibrary.org/obo/GAZ_02000765 -->

    <owl:NamedIndividual rdf:about="http://purl.obolibrary.org/obo/GAZ_02000765"/>
    


    <!-- http://purl.obolibrary.org/obo/GAZ_02000766 -->

    <owl:NamedIndividual rdf:about="http://purl.obolibrary.org/obo/GAZ_02000766"/>
    


    <!-- 
    ///////////////////////////////////////////////////////////////////////////////////////
    //
    // Annotations
    //
    ///////////////////////////////////////////////////////////////////////////////////////
     -->

    <rdf:Description rdf:about="http://purl.obolibrary.org/obo/GAZ_00009238">
        <oboInOwl:hasOBONamespace>GAZ</oboInOwl:hasOBONamespace>
        <rdfs:label>Province (North Korea)</rdfs:label>
        <oboInOwl:id>GAZ:00009238</oboInOwl:id>
    </rdf:Description>
    <rdf:Description rdf:about="http://purl.obolibrary.org/obo/GAZ_00010088">
        <oboInOwl:hasOBONamespace>GAZ</oboInOwl:hasOBONamespace>
        <rdfs:label>populated place, North Korea</rdfs:label>
        <oboInOwl:id>GAZ:00010088</oboInOwl:id>
    </rdf:Description>
    <rdf:Description rdf:about="http://purl.obolibrary.org/obo/GAZ_00010089">
        <obo:IAO_0000115>The capital city of North Korea, located on the Taedong River. The city was split from the South P&apos;yongan province in 1946. It is administered as a Directly Governed City (Chikhalsi), on the same level as provincial governments.</obo:IAO_0000115>
        <rdfs:label>Pyongyang Directly Governed City</rdfs:label>
        <oboInOwl:hasOBONamespace>GAZ</oboInOwl:hasOBONamespace>
        <oboInOwl:id>GAZ:00010089</oboInOwl:id>
    </rdf:Description>
    <rdf:Description rdf:about="http://purl.obolibrary.org/obo/GAZ_00010090">
        <rdfs:label>Directly Governed City</rdfs:label>
        <oboInOwl:hasOBONamespace>GAZ</oboInOwl:hasOBONamespace>
        <oboInOwl:id>GAZ:00010090</oboInOwl:id>
    </rdf:Description>
    <rdf:Description rdf:about="http://purl.obolibrary.org/obo/GAZ_00027636">
        <rdfs:label>Rason Directly Governed City</rdfs:label>
        <oboInOwl:id>GAZ:00027636</oboInOwl:id>
        <obo:IAO_0000115>A Directly Governed City in North Korea, which borders with Jilin province of China and Primorsky Krai of Russia. The region was split from North Hamgyong Province in 1993.</obo:IAO_0000115>
        <oboInOwl:hasOBONamespace>GAZ</oboInOwl:hasOBONamespace>
    </rdf:Description>
    <rdf:Description rdf:about="http://purl.obolibrary.org/obo/GAZ_00027637">
        <obo:IAO_0000115>A special administrative region (SAR) of North Korea, on the border with China. Established 2002-09 in an area including parts of Sinuiju and the surrounding area. It is not one single contiguous region.</obo:IAO_0000115>
        <oboInOwl:hasOBONamespace>GAZ</oboInOwl:hasOBONamespace>
        <oboInOwl:id>GAZ:00027637</oboInOwl:id>
        <rdfs:label>Sinuiju Special Administrative Region</rdfs:label>
    </rdf:Description>
    <rdf:Description rdf:about="http://purl.obolibrary.org/obo/GAZ_00027773">
        <oboInOwl:hasOBONamespace>GAZ</oboInOwl:hasOBONamespace>
        <rdfs:label>Ryongyon County</rdfs:label>
        <oboInOwl:id>GAZ:00027773</oboInOwl:id>
        <obo:IAO_0000115>A county in western Hwanghae-nam Province, North Korea.</obo:IAO_0000115>
    </rdf:Description>
    <rdf:Description rdf:about="http://purl.obolibrary.org/obo/GAZ_00052996">
        <rdfs:label>Pujon</rdfs:label>
        <oboInOwl:hasOBONamespace>GAZ</oboInOwl:hasOBONamespace>
        <oboInOwl:id>GAZ:00052996</oboInOwl:id>
        <obo:IAO_0000115>A populated place. A city in northern South Hamgyong province, North Korea.</obo:IAO_0000115>
    </rdf:Description>
    <rdf:Description rdf:about="http://purl.obolibrary.org/obo/GAZ_00128989">
        <oboInOwl:id>GAZ:00128989</oboInOwl:id>
        <rdfs:label>Yuk-do [Ryongyon]</rdfs:label>
        <oboInOwl:hasOBONamespace>GAZ</oboInOwl:hasOBONamespace>
        <obo:IAO_0000115>An island in Ryongyon County, North Korea.</obo:IAO_0000115>
    </rdf:Description>
    <rdf:Description rdf:about="http://purl.obolibrary.org/obo/GAZ_00128990">
        <rdfs:label>Wollae-do</rdfs:label>
        <oboInOwl:hasOBONamespace>GAZ</oboInOwl:hasOBONamespace>
        <oboInOwl:id>GAZ:00128990</oboInOwl:id>
        <obo:IAO_0000115>An island in Ryongyon County, North Korea.</obo:IAO_0000115>
    </rdf:Description>
    <rdf:Description rdf:about="http://purl.obolibrary.org/obo/GAZ_00128991">
        <obo:IAO_0000115>An island in Ryongyon County, North Korea.</obo:IAO_0000115>
        <oboInOwl:hasOBONamespace>GAZ</oboInOwl:hasOBONamespace>
        <oboInOwl:id>GAZ:00128991</oboInOwl:id>
        <rdfs:label>Ojak-do</rdfs:label>
    </rdf:Description>
    <rdf:Description rdf:about="http://purl.obolibrary.org/obo/GAZ_02000758">
        <oboInOwl:hasOBONamespace>GAZ</oboInOwl:hasOBONamespace>
        <obo:IAO_0000115>A province of North Korea, with its capital at Wonsan. Before the division of Korea in 1945, Kangwo n and its South Korean neighbour Gangwon-do (also spelled Kangwon-do) formed a single province that excluded Wonsan. The province is bordered by South Hamgyong to the north, South P&apos;yongan and North Hwanghae to the west, and Kaesong to the south. Additionally, the province is across the Korean Demilitarized Zone from its South Korean counterpart Gangwon. To the east is the Sea of Japan (East Sea of Korea).</obo:IAO_0000115>
        <oboInOwl:id>GAZ:02000758</oboInOwl:id>
        <rdfs:label>Kangwon Province</rdfs:label>
    </rdf:Description>
    <rdf:Description rdf:about="http://purl.obolibrary.org/obo/GAZ_02000759">
        <oboInOwl:hasOBONamespace>GAZ</oboInOwl:hasOBONamespace>
        <rdfs:label>P&apos;yongan-buk Province</rdfs:label>
        <obo:IAO_0000115>A province of North Korea. The province was formed in 1896 from the northern half of the former P&apos;yongan Province, remained a province of Korea until 1945, then became a province of North Korea. Its capital is Sinuiju. In 2002, Sinuiju Special Administrative Region, near the city of Sinuiju, was established as a separately governed Special Administrative Region. The Yalu River forms the northern border with China. The province is also bordered on the east by Chagang and on the south by South P&apos;yongan. Sinuiju Special Administrative Region (Sinuiju T&apos;ukpyol Haengjonggu) is located in the western corner of the province, and was created as an administrative entity separate from North P&apos;yongan in 2002. North P&apos;yongan is bounded by water on the west with Korea Bay and the Yellow Sea (called the West Sea by Koreans).</obo:IAO_0000115>
        <oboInOwl:id>GAZ:02000759</oboInOwl:id>
    </rdf:Description>
    <rdf:Description rdf:about="http://purl.obolibrary.org/obo/GAZ_02000760">
        <oboInOwl:id>GAZ:02000760</oboInOwl:id>
        <rdfs:label>Chagang Province</rdfs:label>
        <oboInOwl:hasOBONamespace>GAZ</oboInOwl:hasOBONamespace>
        <obo:IAO_0000115>A province in North Korea. The province is bordered by China on the north, Ryanggang and South Hamgyong on the east, South P&apos;yongan on the south, and North P&apos;yongan to the west. Chagang was formed in 1949, when it was separated from North P&apos;yongan. The provincial capital is Kanggye.</obo:IAO_0000115>
    </rdf:Description>
    <rdf:Description rdf:about="http://purl.obolibrary.org/obo/GAZ_02000761">
        <oboInOwl:id>GAZ:02000761</oboInOwl:id>
        <rdfs:label>Hwanghae-nam Province</rdfs:label>
        <oboInOwl:hasOBONamespace>GAZ</oboInOwl:hasOBONamespace>
        <obo:IAO_0000115>A province of North Korea. The province was formed in 1954 when the former Hwanghae Province was split into North and South Hwanghae. The provincial capital is Haeju. It is bordered to the north and east by North Hwanghae province and to the southeast by Kaesong. The southern border of the province is marked by the Korean Demilitarized Zone with South Korea. To the west lies the Yellow Sea.</obo:IAO_0000115>
    </rdf:Description>
    <rdf:Description rdf:about="http://purl.obolibrary.org/obo/GAZ_02000762">
        <oboInOwl:id>GAZ:02000762</oboInOwl:id>
        <oboInOwl:hasOBONamespace>GAZ</oboInOwl:hasOBONamespace>
        <obo:IAO_0000115>A province in North Korea. The province is bordered by China on the north, North Hamgyong on the east, South Hamgyong on the south, and Chagang on the west. Ryanggang was formed in 1954, when it was separated from South Hamgyong. The provincial capital is Hyesan.</obo:IAO_0000115>
        <rdfs:label>Yanggang Province</rdfs:label>
    </rdf:Description>
    <rdf:Description rdf:about="http://purl.obolibrary.org/obo/GAZ_02000763">
        <oboInOwl:id>GAZ:02000763</oboInOwl:id>
        <oboInOwl:hasOBONamespace>GAZ</oboInOwl:hasOBONamespace>
        <rdfs:label>Hamgyong-buk Province</rdfs:label>
        <obo:IAO_0000115>A province of North Korea. The province was formed in 1896 from the northern half of the former Hamgyong Province, remained a province of Korea until 1945, then became a province of North Korea. Its capital is Ch&apos;ongjin. The province is bordered by China on the north, South Hamgyong on the southwest, and Ryanggang on the west. On the east is the Sea of Japan (East Sea of Korea). There is also a short border with Russia.</obo:IAO_0000115>
    </rdf:Description>
    <rdf:Description rdf:about="http://purl.obolibrary.org/obo/GAZ_02000764">
        <obo:IAO_0000115>A province of North Korea. The province was formed in 1954 when the former Hwanghae Province was split into North and South Hwanghae. The provincial capital is Sariwon. The province is bordered by P&apos;yongyang and South P&apos;yongan to the north, Kangwon to the east, Kaesong Industrial Region to the south, and South Hwanghae southwest. In 2003, Kaesong Directly Governed City (Kaesong Chikhalsi) became part of North Hwanghae.</obo:IAO_0000115>
        <rdfs:label>Hwanghae-buk Province</rdfs:label>
        <oboInOwl:hasOBONamespace>GAZ</oboInOwl:hasOBONamespace>
        <oboInOwl:id>GAZ:02000764</oboInOwl:id>
    </rdf:Description>
    <rdf:Description rdf:about="http://purl.obolibrary.org/obo/GAZ_02000765">
        <oboInOwl:hasOBONamespace>GAZ</oboInOwl:hasOBONamespace>
        <obo:IAO_0000115>A province of North Korea. The province was formed in 1896 from the southern half of the former P&apos;yongan Province, remained a province of Korea until 1945, then became a province of North Korea. Its capital is P&apos;yongsong. The province is bordered by North P&apos;yongan and Chagang to the north, South Hamgyong and Kangwon to the east and southeast, and North Hwanghae and P&apos;yongyang to the south. The Yellow Sea and Korea Bay are located to the west.</obo:IAO_0000115>
        <oboInOwl:id>GAZ:02000765</oboInOwl:id>
        <rdfs:label>P&apos;yongan-nam Province</rdfs:label>
    </rdf:Description>
    <rdf:Description rdf:about="http://purl.obolibrary.org/obo/GAZ_02000766">
        <oboInOwl:id>GAZ:02000766</oboInOwl:id>
        <rdfs:label>Hamgyong-nam Province</rdfs:label>
        <obo:IAO_0000115>A province of North Korea. The province was formed in 1896 from the southern half of the former Hamgyong Province, remained a province of Korea until 1945, then became a province of North Korea. Its capital is Hamhung. The province is bordered by Ryanggang to the north, North Hamgyong to the northeast, Kangwon to the south, and South P&apos;yongan to the west. On the east of the province is the Sea of Japan (East Sea of Korea).</obo:IAO_0000115>
        <oboInOwl:hasOBONamespace>GAZ</oboInOwl:hasOBONamespace>
    </rdf:Description>
</rdf:RDF>



<!-- Generated by the OWL API (version 4.5.6) https://github.com/owlcs/owlapi -->

