<?xml version="1.0"?>
<rdf:RDF xmlns="http://purl.obolibrary.org/obo/gaz/subsets/countries/Pakistan.owl#"
     xml:base="http://purl.obolibrary.org/obo/gaz/subsets/countries/Pakistan.owl"
     xmlns:obo="http://purl.obolibrary.org/obo/"
     xmlns:owl="http://www.w3.org/2002/07/owl#"
     xmlns:rdf="http://www.w3.org/1999/02/22-rdf-syntax-ns#"
     xmlns:xml="http://www.w3.org/XML/1998/namespace"
     xmlns:xsd="http://www.w3.org/2001/XMLSchema#"
     xmlns:rdfs="http://www.w3.org/2000/01/rdf-schema#"
     xmlns:oboInOwl="http://www.geneontology.org/formats/oboInOwl#">
    <owl:Ontology rdf:about="http://purl.obolibrary.org/obo/gaz/subsets/countries/Pakistan.owl">
        <owl:imports rdf:resource="http://purl.obolibrary.org/obo/gaz/imports/envo_import.owl"/>
        <owl:imports rdf:resource="http://purl.obolibrary.org/obo/gaz/imports/ro_import.owl"/>
    </owl:Ontology>
    


    <!-- 
    ///////////////////////////////////////////////////////////////////////////////////////
    //
    // Annotation properties
    //
    ///////////////////////////////////////////////////////////////////////////////////////
     -->

    


    <!-- http://purl.obolibrary.org/obo/IAO_0000115 -->

    <owl:AnnotationProperty rdf:about="http://purl.obolibrary.org/obo/IAO_0000115"/>
    


    <!-- http://www.geneontology.org/formats/oboInOwl#hasOBONamespace -->

    <owl:AnnotationProperty rdf:about="http://www.geneontology.org/formats/oboInOwl#hasOBONamespace"/>
    


    <!-- http://www.geneontology.org/formats/oboInOwl#id -->

    <owl:AnnotationProperty rdf:about="http://www.geneontology.org/formats/oboInOwl#id"/>
    


    <!-- 
    ///////////////////////////////////////////////////////////////////////////////////////
    //
    // Object Properties
    //
    ///////////////////////////////////////////////////////////////////////////////////////
     -->

    


    <!-- http://purl.obolibrary.org/obo/RO_0001025 -->

    <owl:ObjectProperty rdf:about="http://purl.obolibrary.org/obo/RO_0001025"/>
    


    <!-- 
    ///////////////////////////////////////////////////////////////////////////////////////
    //
    // Classes
    //
    ///////////////////////////////////////////////////////////////////////////////////////
     -->

    


    <!-- http://purl.obolibrary.org/obo/ENVO_00000004 -->

    <owl:Class rdf:about="http://purl.obolibrary.org/obo/ENVO_00000004"/>
    


    <!-- http://purl.obolibrary.org/obo/ENVO_00000009 -->

    <owl:Class rdf:about="http://purl.obolibrary.org/obo/ENVO_00000009"/>
    


    <!-- http://purl.obolibrary.org/obo/ENVO_00000074 -->

    <owl:Class rdf:about="http://purl.obolibrary.org/obo/ENVO_00000074"/>
    


    <!-- http://purl.obolibrary.org/obo/ENVO_00000100 -->

    <owl:Class rdf:about="http://purl.obolibrary.org/obo/ENVO_00000100"/>
    


    <!-- http://purl.obolibrary.org/obo/ENVO_00000104 -->

    <owl:Class rdf:about="http://purl.obolibrary.org/obo/ENVO_00000104"/>
    


    <!-- http://purl.obolibrary.org/obo/ENVO_00000106 -->

    <owl:Class rdf:about="http://purl.obolibrary.org/obo/ENVO_00000106"/>
    


    <!-- http://purl.obolibrary.org/obo/ENVO_00000856 -->

    <owl:Class rdf:about="http://purl.obolibrary.org/obo/ENVO_00000856"/>
    


    <!-- http://purl.obolibrary.org/obo/GAZ_00005247 -->

    <owl:Class rdf:about="http://purl.obolibrary.org/obo/GAZ_00005247"/>
    


    <!-- http://purl.obolibrary.org/obo/GAZ_00005248 -->

    <owl:Class rdf:about="http://purl.obolibrary.org/obo/GAZ_00005248">
        <rdfs:subClassOf rdf:resource="http://purl.obolibrary.org/obo/GAZ_00005247"/>
    </owl:Class>
    


    <!-- http://purl.obolibrary.org/obo/GAZ_00005249 -->

    <owl:Class rdf:about="http://purl.obolibrary.org/obo/GAZ_00005249">
        <rdfs:subClassOf rdf:resource="http://purl.obolibrary.org/obo/GAZ_00005247"/>
    </owl:Class>
    


    <!-- http://purl.obolibrary.org/obo/GAZ_00005250 -->

    <owl:Class rdf:about="http://purl.obolibrary.org/obo/GAZ_00005250">
        <rdfs:subClassOf rdf:resource="http://purl.obolibrary.org/obo/GAZ_00005247"/>
    </owl:Class>
    


    <!-- http://purl.obolibrary.org/obo/GAZ_00005251 -->

    <owl:Class rdf:about="http://purl.obolibrary.org/obo/GAZ_00005251">
        <rdfs:subClassOf rdf:resource="http://purl.obolibrary.org/obo/GAZ_00005247"/>
    </owl:Class>
    


    <!-- http://purl.obolibrary.org/obo/GAZ_00005252 -->

    <owl:Class rdf:about="http://purl.obolibrary.org/obo/GAZ_00005252"/>
    


    <!-- http://purl.obolibrary.org/obo/GAZ_00005253 -->

    <owl:Class rdf:about="http://purl.obolibrary.org/obo/GAZ_00005253">
        <rdfs:subClassOf rdf:resource="http://purl.obolibrary.org/obo/GAZ_00005252"/>
    </owl:Class>
    


    <!-- http://purl.obolibrary.org/obo/GAZ_00005254 -->

    <owl:Class rdf:about="http://purl.obolibrary.org/obo/GAZ_00005254">
        <rdfs:subClassOf rdf:resource="http://purl.obolibrary.org/obo/GAZ_00005252"/>
    </owl:Class>
    


    <!-- http://purl.obolibrary.org/obo/GAZ_00005255 -->

    <owl:Class rdf:about="http://purl.obolibrary.org/obo/GAZ_00005255">
        <rdfs:subClassOf rdf:resource="http://purl.obolibrary.org/obo/GAZ_00005252"/>
    </owl:Class>
    


    <!-- http://purl.obolibrary.org/obo/GAZ_00005258 -->

    <owl:Class rdf:about="http://purl.obolibrary.org/obo/GAZ_00005258"/>
    


    <!-- http://purl.obolibrary.org/obo/GAZ_00005259 -->

    <owl:Class rdf:about="http://purl.obolibrary.org/obo/GAZ_00005259">
        <rdfs:subClassOf rdf:resource="http://purl.obolibrary.org/obo/GAZ_00005258"/>
    </owl:Class>
    


    <!-- http://purl.obolibrary.org/obo/GAZ_00007411 -->

    <owl:Class rdf:about="http://purl.obolibrary.org/obo/GAZ_00007411">
        <rdfs:subClassOf rdf:resource="http://purl.obolibrary.org/obo/GAZ_00005258"/>
    </owl:Class>
    


    <!-- http://purl.obolibrary.org/obo/GAZ_00007535 -->

    <owl:Class rdf:about="http://purl.obolibrary.org/obo/GAZ_00007535">
        <rdfs:subClassOf rdf:resource="http://purl.obolibrary.org/obo/GAZ_00005258"/>
    </owl:Class>
    


    <!-- http://purl.obolibrary.org/obo/GAZ_00010428 -->

    <owl:Class rdf:about="http://purl.obolibrary.org/obo/GAZ_00010428">
        <rdfs:subClassOf rdf:resource="http://purl.obolibrary.org/obo/GAZ_00005258"/>
    </owl:Class>
    


    <!-- http://purl.obolibrary.org/obo/GAZ_00058448 -->

    <owl:Class rdf:about="http://purl.obolibrary.org/obo/GAZ_00058448">
        <rdfs:subClassOf rdf:resource="http://purl.obolibrary.org/obo/GAZ_00005258"/>
    </owl:Class>
    


    <!-- http://purl.obolibrary.org/obo/GAZ_00058473 -->

    <owl:Class rdf:about="http://purl.obolibrary.org/obo/GAZ_00058473">
        <rdfs:subClassOf rdf:resource="http://purl.obolibrary.org/obo/GAZ_00005258"/>
    </owl:Class>
    


    <!-- http://purl.obolibrary.org/obo/GAZ_00080184 -->

    <owl:Class rdf:about="http://purl.obolibrary.org/obo/GAZ_00080184">
        <rdfs:subClassOf rdf:resource="http://purl.obolibrary.org/obo/GAZ_00005258"/>
    </owl:Class>
    


    <!-- http://purl.obolibrary.org/obo/GAZ_00080452 -->

    <owl:Class rdf:about="http://purl.obolibrary.org/obo/GAZ_00080452">
        <rdfs:subClassOf rdf:resource="http://purl.obolibrary.org/obo/GAZ_00005258"/>
    </owl:Class>
    


    <!-- http://purl.obolibrary.org/obo/GAZ_22223590 -->

    <owl:Class rdf:about="http://purl.obolibrary.org/obo/GAZ_22223590">
        <rdfs:subClassOf rdf:resource="http://purl.obolibrary.org/obo/GAZ_00005258"/>
    </owl:Class>
    


    <!-- http://purl.obolibrary.org/obo/GAZ_22223591 -->

    <owl:Class rdf:about="http://purl.obolibrary.org/obo/GAZ_22223591">
        <rdfs:subClassOf rdf:resource="http://purl.obolibrary.org/obo/GAZ_00005258"/>
    </owl:Class>
    


    <!-- 
    ///////////////////////////////////////////////////////////////////////////////////////
    //
    // Individuals
    //
    ///////////////////////////////////////////////////////////////////////////////////////
     -->

    


    <!-- http://purl.obolibrary.org/obo/GAZ_00004988 -->

    <owl:NamedIndividual rdf:about="http://purl.obolibrary.org/obo/GAZ_00004988">
        <obo:RO_0001025 rdf:resource="http://purl.obolibrary.org/obo/GAZ_00005246"/>
        <obo:IAO_0000115>A mountain range located in Central Asia and are formed by the junction or knot of the Tian Shan, Karakoram, Kunlun, and Hindu Kush ranges. The Pamir region is centered in the Tajikistani region of Gorno-Badakhshan. Parts of the Pamir also lie in the countries of Kyrgyzstan, Afghanistan, and Pakistan. South of Gorno-Badakhshan, the Wakhan Corridor runs through the Pamir region, which also includes the northern extremes of the North-West Frontier Province and the northern extremes of the Northern Areas of Pakistan.</obo:IAO_0000115>
        <oboInOwl:hasOBONamespace>GAZ</oboInOwl:hasOBONamespace>
        <oboInOwl:id>GAZ:00004988</oboInOwl:id>
        <rdfs:label>Pamir Mountains</rdfs:label>
    </owl:NamedIndividual>
    


    <!-- http://purl.obolibrary.org/obo/GAZ_00005246 -->

    <owl:NamedIndividual rdf:about="http://purl.obolibrary.org/obo/GAZ_00005246">
        <rdf:type rdf:resource="http://purl.obolibrary.org/obo/ENVO_00000009"/>
        <obo:IAO_0000115>A country in Middle East which lies on the Iranian Plateau and some parts of South Asia. It is located in the region where South Asia converges with Central Asia and the Middle East. It has a 1,046 km coastline along the Arabian Sea in the south, and is bordered by Afghanistan and Iran in the west, India in the east and China in the far northeast. Pakistan is subdivided into four provinces and two territories. In addition, the portion of Kashmir that is administered by the Pakistani government is divided into two separate administrative units. The provinces are divided into a total of 105 zillas (districts). A zilla is further subdivided into tehsils (roughly equivalent to counties). Tehsils may contain villages or municipalities. There are over five thousand local governments in Pakistan.</obo:IAO_0000115>
        <oboInOwl:hasOBONamespace>GAZ</oboInOwl:hasOBONamespace>
        <oboInOwl:id>GAZ:00005246</oboInOwl:id>
        <rdfs:label>Pakistan</rdfs:label>
    </owl:NamedIndividual>
    


    <!-- http://purl.obolibrary.org/obo/GAZ_00005247 -->

    <owl:NamedIndividual rdf:about="http://purl.obolibrary.org/obo/GAZ_00005247">
        <obo:RO_0001025 rdf:resource="http://purl.obolibrary.org/obo/GAZ_00005246"/>
    </owl:NamedIndividual>
    


    <!-- http://purl.obolibrary.org/obo/GAZ_00005248 -->

    <owl:NamedIndividual rdf:about="http://purl.obolibrary.org/obo/GAZ_00005248"/>
    


    <!-- http://purl.obolibrary.org/obo/GAZ_00005249 -->

    <owl:NamedIndividual rdf:about="http://purl.obolibrary.org/obo/GAZ_00005249"/>
    


    <!-- http://purl.obolibrary.org/obo/GAZ_00005250 -->

    <owl:NamedIndividual rdf:about="http://purl.obolibrary.org/obo/GAZ_00005250"/>
    


    <!-- http://purl.obolibrary.org/obo/GAZ_00005251 -->

    <owl:NamedIndividual rdf:about="http://purl.obolibrary.org/obo/GAZ_00005251"/>
    


    <!-- http://purl.obolibrary.org/obo/GAZ_00005252 -->

    <owl:NamedIndividual rdf:about="http://purl.obolibrary.org/obo/GAZ_00005252">
        <obo:RO_0001025 rdf:resource="http://purl.obolibrary.org/obo/GAZ_00005246"/>
    </owl:NamedIndividual>
    


    <!-- http://purl.obolibrary.org/obo/GAZ_00005253 -->

    <owl:NamedIndividual rdf:about="http://purl.obolibrary.org/obo/GAZ_00005253"/>
    


    <!-- http://purl.obolibrary.org/obo/GAZ_00005254 -->

    <owl:NamedIndividual rdf:about="http://purl.obolibrary.org/obo/GAZ_00005254"/>
    


    <!-- http://purl.obolibrary.org/obo/GAZ_00005255 -->

    <owl:NamedIndividual rdf:about="http://purl.obolibrary.org/obo/GAZ_00005255"/>
    


    <!-- http://purl.obolibrary.org/obo/GAZ_00005256 -->

    <owl:NamedIndividual rdf:about="http://purl.obolibrary.org/obo/GAZ_00005256">
        <obo:RO_0001025 rdf:resource="http://purl.obolibrary.org/obo/GAZ_00005255"/>
        <obo:IAO_0000115>The northernmost political entity within the Pakistani-controlled part of the former princely State of Jammu and Kashmir. It borders Pakistan to the west, Afghanistan to the north, China to the northeast, the Pakistani-controlled State of Azad Jammu and Kashmir (AJK) to the south, and the present-day Indian State of Jammu and Kashmir to the southeast. The Northern Areas, which became a single administrative unit in 1970, was formed from the amalgamation of the Gilgit Agency, the Baltistan District of the Ladakh Wazarat, and the states of Hunza and Nagar.</obo:IAO_0000115>
        <oboInOwl:hasOBONamespace>GAZ</oboInOwl:hasOBONamespace>
        <oboInOwl:id>GAZ:00005256</oboInOwl:id>
        <rdfs:label>Federally Administered Northern Areas</rdfs:label>
    </owl:NamedIndividual>
    


    <!-- http://purl.obolibrary.org/obo/GAZ_00005257 -->

    <owl:NamedIndividual rdf:about="http://purl.obolibrary.org/obo/GAZ_00005257">
        <obo:RO_0001025 rdf:resource="http://purl.obolibrary.org/obo/GAZ_00005255"/>
        <obo:IAO_0000115>The southernmost political entity of the Pakistani-controlled part of the former princely State of Jammu and Kashmir. It borders the present-day Indian-annexed State of Jammu and Kashmir to the east, the Federally Administered Northern Areas (FANA) to the north, and the North-West Frontier Province of Pakistan to the west. Azad Jammu and Kashmir (AJK) is a self-governing state under Pakistani control. The state is divided into two administrative divisions which, in turn, are composed of a total of eight districts.</obo:IAO_0000115>
        <oboInOwl:hasOBONamespace>GAZ</oboInOwl:hasOBONamespace>
        <oboInOwl:id>GAZ:00005257</oboInOwl:id>
        <rdfs:label>State of Azad Kashmir</rdfs:label>
    </owl:NamedIndividual>
    


    <!-- http://purl.obolibrary.org/obo/GAZ_00005258 -->

    <owl:NamedIndividual rdf:about="http://purl.obolibrary.org/obo/GAZ_00005258">
        <obo:RO_0001025 rdf:resource="http://purl.obolibrary.org/obo/GAZ_00005246"/>
    </owl:NamedIndividual>
    


    <!-- http://purl.obolibrary.org/obo/GAZ_00005259 -->

    <owl:NamedIndividual rdf:about="http://purl.obolibrary.org/obo/GAZ_00005259">
        <obo:RO_0001025 rdf:resource="http://purl.obolibrary.org/obo/GAZ_00009470"/>
    </owl:NamedIndividual>
    


    <!-- http://purl.obolibrary.org/obo/GAZ_00005260 -->

    <owl:NamedIndividual rdf:about="http://purl.obolibrary.org/obo/GAZ_00005260">
        <obo:RO_0001025 rdf:resource="http://purl.obolibrary.org/obo/GAZ_00080488"/>
        <obo:IAO_0000115>A planted forest in Pakistan. It is located in Chunian is about 70 km south of Lahore. It covers an area of 50 km2 and is one of the largest of its kind. The planting and irrigation of it took place in the 19th century in the era of the British Raj due to the need for timber for the Indian railway network.</obo:IAO_0000115>
        <oboInOwl:hasOBONamespace>GAZ</oboInOwl:hasOBONamespace>
        <oboInOwl:id>GAZ:00005260</oboInOwl:id>
        <rdfs:label>Changa Manga Forest</rdfs:label>
    </owl:NamedIndividual>
    


    <!-- http://purl.obolibrary.org/obo/GAZ_00007411 -->

    <owl:NamedIndividual rdf:about="http://purl.obolibrary.org/obo/GAZ_00007411">
        <obo:RO_0001025 rdf:resource="http://purl.obolibrary.org/obo/GAZ_00009471"/>
    </owl:NamedIndividual>
    


    <!-- http://purl.obolibrary.org/obo/GAZ_00007534 -->

    <owl:NamedIndividual rdf:about="http://purl.obolibrary.org/obo/GAZ_00007534">
        <rdf:type rdf:resource="http://purl.obolibrary.org/obo/ENVO_00000004"/>
        <obo:RO_0001025 rdf:resource="http://purl.obolibrary.org/obo/GAZ_00005249"/>
        <obo:IAO_0000115>A district in the Punjab province of Pakistan.</obo:IAO_0000115>
        <oboInOwl:hasOBONamespace>GAZ</oboInOwl:hasOBONamespace>
        <oboInOwl:id>GAZ:00007534</oboInOwl:id>
        <rdfs:label>Dera Ghazi Khan District</rdfs:label>
    </owl:NamedIndividual>
    


    <!-- http://purl.obolibrary.org/obo/GAZ_00007535 -->

    <owl:NamedIndividual rdf:about="http://purl.obolibrary.org/obo/GAZ_00007535">
        <obo:RO_0001025 rdf:resource="http://purl.obolibrary.org/obo/GAZ_00080490"/>
    </owl:NamedIndividual>
    


    <!-- http://purl.obolibrary.org/obo/GAZ_00008310 -->

    <owl:NamedIndividual rdf:about="http://purl.obolibrary.org/obo/GAZ_00008310">
        <obo:RO_0001025 rdf:resource="http://purl.obolibrary.org/obo/GAZ_00004988"/>
        <oboInOwl:hasOBONamespace>GAZ</oboInOwl:hasOBONamespace>
        <oboInOwl:id>GAZ:00008310</oboInOwl:id>
        <rdfs:label>East Pamirs</rdfs:label>
    </owl:NamedIndividual>
    


    <!-- http://purl.obolibrary.org/obo/GAZ_00009470 -->

    <owl:NamedIndividual rdf:about="http://purl.obolibrary.org/obo/GAZ_00009470">
        <rdf:type rdf:resource="http://purl.obolibrary.org/obo/ENVO_00000004"/>
        <obo:RO_0001025 rdf:resource="http://purl.obolibrary.org/obo/GAZ_00005249"/>
        <obo:IAO_0000115>A district in the Punjab province of Pakistan, that contains the city of Lahore - the district and provincial capital.</obo:IAO_0000115>
        <oboInOwl:hasOBONamespace>GAZ</oboInOwl:hasOBONamespace>
        <oboInOwl:id>GAZ:00009470</oboInOwl:id>
        <rdfs:label>Lahore District</rdfs:label>
    </owl:NamedIndividual>
    


    <!-- http://purl.obolibrary.org/obo/GAZ_00009471 -->

    <owl:NamedIndividual rdf:about="http://purl.obolibrary.org/obo/GAZ_00009471">
        <obo:RO_0001025 rdf:resource="http://purl.obolibrary.org/obo/GAZ_00005251"/>
        <oboInOwl:hasOBONamespace>GAZ</oboInOwl:hasOBONamespace>
        <oboInOwl:id>GAZ:00009471</oboInOwl:id>
        <rdfs:label>Karachi District</rdfs:label>
    </owl:NamedIndividual>
    


    <!-- http://purl.obolibrary.org/obo/GAZ_00010428 -->

    <owl:NamedIndividual rdf:about="http://purl.obolibrary.org/obo/GAZ_00010428">
        <obo:RO_0001025 rdf:resource="http://purl.obolibrary.org/obo/GAZ_00005254"/>
    </owl:NamedIndividual>
    


    <!-- http://purl.obolibrary.org/obo/GAZ_00010429 -->

    <owl:NamedIndividual rdf:about="http://purl.obolibrary.org/obo/GAZ_00010429">
        <obo:RO_0001025 rdf:resource="http://purl.obolibrary.org/obo/GAZ_00012614"/>
        <obo:IAO_0000115>One of the seven Tehsils of Rawalpindi District in the Punjab province of Pakistan.</obo:IAO_0000115>
        <oboInOwl:hasOBONamespace>GAZ</oboInOwl:hasOBONamespace>
        <oboInOwl:id>GAZ:00010429</oboInOwl:id>
        <rdfs:label>Rawalpindi Tehsil</rdfs:label>
    </owl:NamedIndividual>
    


    <!-- http://purl.obolibrary.org/obo/GAZ_00011784 -->

    <owl:NamedIndividual rdf:about="http://purl.obolibrary.org/obo/GAZ_00011784">
        <obo:RO_0001025 rdf:resource="http://purl.obolibrary.org/obo/GAZ_00057344"/>
        <obo:IAO_0000115>A mountain of the Himalaya range in High Asia, is located on the border between Nepal and Tibet, China.</obo:IAO_0000115>
        <oboInOwl:hasOBONamespace>GAZ</oboInOwl:hasOBONamespace>
        <oboInOwl:id>GAZ:00011784</oboInOwl:id>
        <rdfs:label>Mount Everest</rdfs:label>
    </owl:NamedIndividual>
    


    <!-- http://purl.obolibrary.org/obo/GAZ_00012614 -->

    <owl:NamedIndividual rdf:about="http://purl.obolibrary.org/obo/GAZ_00012614">
        <rdf:type rdf:resource="http://purl.obolibrary.org/obo/ENVO_00000004"/>
        <obo:RO_0001025 rdf:resource="http://purl.obolibrary.org/obo/GAZ_00005249"/>
        <obo:IAO_0000115>A district of Pakistan in the north of the Punjab province which contains the city of Rawalpindi.</obo:IAO_0000115>
        <oboInOwl:hasOBONamespace>GAZ</oboInOwl:hasOBONamespace>
        <oboInOwl:id>GAZ:00012614</oboInOwl:id>
        <rdfs:label>Rawalpindi District</rdfs:label>
    </owl:NamedIndividual>
    


    <!-- http://purl.obolibrary.org/obo/GAZ_00018488 -->

    <owl:NamedIndividual rdf:about="http://purl.obolibrary.org/obo/GAZ_00018488">
        <rdf:type rdf:resource="http://purl.obolibrary.org/obo/ENVO_00000004"/>
        <obo:RO_0001025 rdf:resource="http://purl.obolibrary.org/obo/GAZ_00005248"/>
        <obo:IAO_0000115>A district of Balochistan.</obo:IAO_0000115>
        <oboInOwl:hasOBONamespace>GAZ</oboInOwl:hasOBONamespace>
        <oboInOwl:id>GAZ:00018488</oboInOwl:id>
        <rdfs:label>Gwadar District</rdfs:label>
    </owl:NamedIndividual>
    


    <!-- http://purl.obolibrary.org/obo/GAZ_00018489 -->

    <owl:NamedIndividual rdf:about="http://purl.obolibrary.org/obo/GAZ_00018489">
        <obo:RO_0001025 rdf:resource="http://purl.obolibrary.org/obo/GAZ_00080188"/>
        <obo:IAO_0000115>A small, uninhabited island in the Arabian Sea, some 40 km East-South-East of the Pakistani fishing port of Pasni, Balochistan.</obo:IAO_0000115>
        <oboInOwl:hasOBONamespace>GAZ</oboInOwl:hasOBONamespace>
        <oboInOwl:id>GAZ:00018489</oboInOwl:id>
        <rdfs:label>Astola Island</rdfs:label>
    </owl:NamedIndividual>
    


    <!-- http://purl.obolibrary.org/obo/GAZ_00018490 -->

    <owl:NamedIndividual rdf:about="http://purl.obolibrary.org/obo/GAZ_00018490">
        <obo:RO_0001025 rdf:resource="http://purl.obolibrary.org/obo/GAZ_00007411"/>
        <obo:IAO_0000115>The main coastal town of Karachi, located in the central and western parts of the city, including the Port of Karachi and an extensive coastline with sandy beaches, small islands and mangrove forests. It does not include the southern island of Manora which is under cantonment administration because of the naval base located there. The town forms a large triangle with highly defined boundaries - the RCD Highway and the Lyari River forming the northeastern border, the Hub River forming the northwestern border and the Arabian Sea forming the southern border.</obo:IAO_0000115>
        <oboInOwl:hasOBONamespace>GAZ</oboInOwl:hasOBONamespace>
        <oboInOwl:id>GAZ:00018490</oboInOwl:id>
        <rdfs:label>Kiamari Town</rdfs:label>
    </owl:NamedIndividual>
    


    <!-- http://purl.obolibrary.org/obo/GAZ_00018491 -->

    <owl:NamedIndividual rdf:about="http://purl.obolibrary.org/obo/GAZ_00018491">
        <obo:RO_0001025 rdf:resource="http://purl.obolibrary.org/obo/GAZ_00018490"/>
        <obo:IAO_0000115>The smallest neighborhood of Kiamari Town in Karachi, Sindh, Pakistan. It comprises three small fishing islands which in the centre of the harbour of Karachi.</obo:IAO_0000115>
        <oboInOwl:hasOBONamespace>GAZ</oboInOwl:hasOBONamespace>
        <oboInOwl:id>GAZ:00018491</oboInOwl:id>
        <rdfs:label>Bhit Shah Island</rdfs:label>
    </owl:NamedIndividual>
    


    <!-- http://purl.obolibrary.org/obo/GAZ_00018492 -->

    <owl:NamedIndividual rdf:about="http://purl.obolibrary.org/obo/GAZ_00018492">
        <obo:RO_0001025 rdf:resource="http://purl.obolibrary.org/obo/GAZ_00009471"/>
        <obo:IAO_0000115>A small island located in the Arabian Sea off the coast of Karachi, Sindh, Pakistan.</obo:IAO_0000115>
        <oboInOwl:hasOBONamespace>GAZ</oboInOwl:hasOBONamespace>
        <oboInOwl:id>GAZ:00018492</oboInOwl:id>
        <rdfs:label>Buddo Island</rdfs:label>
    </owl:NamedIndividual>
    


    <!-- http://purl.obolibrary.org/obo/GAZ_00018493 -->

    <owl:NamedIndividual rdf:about="http://purl.obolibrary.org/obo/GAZ_00018493">
        <obo:RO_0001025 rdf:resource="http://purl.obolibrary.org/obo/GAZ_00009471"/>
        <obo:IAO_0000115>A small island located in the Arabian Sea off the coast of Karachi, Sindh, Pakistan.</obo:IAO_0000115>
        <oboInOwl:hasOBONamespace>GAZ</oboInOwl:hasOBONamespace>
        <oboInOwl:id>GAZ:00018493</oboInOwl:id>
        <rdfs:label>Bundal Island</rdfs:label>
    </owl:NamedIndividual>
    


    <!-- http://purl.obolibrary.org/obo/GAZ_00018494 -->

    <owl:NamedIndividual rdf:about="http://purl.obolibrary.org/obo/GAZ_00018494">
        <obo:RO_0001025 rdf:resource="http://purl.obolibrary.org/obo/GAZ_00009471"/>
        <obo:IAO_0000115>A small island located in the Arabian Sea off the coast of Karachi, Sindh, Pakistan.</obo:IAO_0000115>
        <oboInOwl:hasOBONamespace>GAZ</oboInOwl:hasOBONamespace>
        <oboInOwl:id>GAZ:00018494</oboInOwl:id>
        <rdfs:label>Churma Island</rdfs:label>
    </owl:NamedIndividual>
    


    <!-- http://purl.obolibrary.org/obo/GAZ_00018495 -->

    <owl:NamedIndividual rdf:about="http://purl.obolibrary.org/obo/GAZ_00018495">
        <obo:RO_0001025 rdf:resource="http://purl.obolibrary.org/obo/GAZ_00007411"/>
        <obo:IAO_0000115>A small densely populated town in the central part of old Karachi. The town is bordered by Jamshed Town and Clifton Cantonment to the east, Kiamari Town and the Arabian Sea to the south and Lyari Town to the west.</obo:IAO_0000115>
        <oboInOwl:hasOBONamespace>GAZ</oboInOwl:hasOBONamespace>
        <oboInOwl:id>GAZ:00018495</oboInOwl:id>
        <rdfs:label>Saddar Town</rdfs:label>
    </owl:NamedIndividual>
    


    <!-- http://purl.obolibrary.org/obo/GAZ_00018496 -->

    <owl:NamedIndividual rdf:about="http://purl.obolibrary.org/obo/GAZ_00018496">
        <obo:RO_0001025 rdf:resource="http://purl.obolibrary.org/obo/GAZ_00018495"/>
        <obo:IAO_0000115>A neighborhood of Saddar Town in Karachi, Sindh, Pakistan. Clifton lies in the southern area of Saddar Town.</obo:IAO_0000115>
        <oboInOwl:hasOBONamespace>GAZ</oboInOwl:hasOBONamespace>
        <oboInOwl:id>GAZ:00018496</oboInOwl:id>
        <rdfs:label>Clifton</rdfs:label>
    </owl:NamedIndividual>
    


    <!-- http://purl.obolibrary.org/obo/GAZ_00018497 -->

    <owl:NamedIndividual rdf:about="http://purl.obolibrary.org/obo/GAZ_00018497">
        <obo:RO_0001025 rdf:resource="http://purl.obolibrary.org/obo/GAZ_00018496"/>
        <oboInOwl:hasOBONamespace>GAZ</oboInOwl:hasOBONamespace>
        <oboInOwl:id>GAZ:00018497</oboInOwl:id>
        <rdfs:label>Clifton Oyster Rocks</rdfs:label>
    </owl:NamedIndividual>
    


    <!-- http://purl.obolibrary.org/obo/GAZ_00018498 -->

    <owl:NamedIndividual rdf:about="http://purl.obolibrary.org/obo/GAZ_00018498">
        <obo:RO_0001025 rdf:resource="http://purl.obolibrary.org/obo/GAZ_00009471"/>
        <obo:IAO_0000115>A small island located in the Arabian Sea off the coast of Karachi, Sindh, Pakistan.</obo:IAO_0000115>
        <oboInOwl:hasOBONamespace>GAZ</oboInOwl:hasOBONamespace>
        <oboInOwl:id>GAZ:00018498</oboInOwl:id>
        <rdfs:label>Khiprianwala Island</rdfs:label>
    </owl:NamedIndividual>
    


    <!-- http://purl.obolibrary.org/obo/GAZ_00018499 -->

    <owl:NamedIndividual rdf:about="http://purl.obolibrary.org/obo/GAZ_00018499">
        <obo:RO_0001025 rdf:resource="http://purl.obolibrary.org/obo/GAZ_00005248"/>
        <obo:IAO_0000115>An offshore mud volcano located in the Arabian Sea, 3 km off the coast of Balochistan, Pakistan. It rose out of the water overnight in 1999-03.</obo:IAO_0000115>
        <oboInOwl:hasOBONamespace>GAZ</oboInOwl:hasOBONamespace>
        <oboInOwl:id>GAZ:00018499</oboInOwl:id>
        <rdfs:label>Malan Island</rdfs:label>
    </owl:NamedIndividual>
    


    <!-- http://purl.obolibrary.org/obo/GAZ_00018500 -->

    <owl:NamedIndividual rdf:about="http://purl.obolibrary.org/obo/GAZ_00018500">
        <obo:RO_0001025 rdf:resource="http://purl.obolibrary.org/obo/GAZ_00080304"/>
        <obo:IAO_0000115>A small island (2.5 km2) located just south of the Port of Karachi, Sindh, Pakistan. The island is connected to the mainland by a 12 km long causeway called the Sandspit. Manora and neighbouring islands form a protective barrier between Karachi harbour to the north and the Arabian Sea to the south. The western bay of the harbour contains endangered mangrove forests which border the Sandspit and Manora island.</obo:IAO_0000115>
        <oboInOwl:hasOBONamespace>GAZ</oboInOwl:hasOBONamespace>
        <oboInOwl:id>GAZ:00018500</oboInOwl:id>
        <rdfs:label>Manora Island</rdfs:label>
    </owl:NamedIndividual>
    


    <!-- http://purl.obolibrary.org/obo/GAZ_00018545 -->

    <owl:NamedIndividual rdf:about="http://purl.obolibrary.org/obo/GAZ_00018545">
        <rdf:type rdf:resource="http://purl.obolibrary.org/obo/ENVO_00000004"/>
        <obo:RO_0001025 rdf:resource="http://purl.obolibrary.org/obo/GAZ_00005251"/>
        <obo:IAO_0000115>A district of Sindh, Pakistan.</obo:IAO_0000115>
        <oboInOwl:hasOBONamespace>GAZ</oboInOwl:hasOBONamespace>
        <oboInOwl:id>GAZ:00018545</oboInOwl:id>
        <rdfs:label>Jacobabad District</rdfs:label>
    </owl:NamedIndividual>
    


    <!-- http://purl.obolibrary.org/obo/GAZ_00018546 -->

    <owl:NamedIndividual rdf:about="http://purl.obolibrary.org/obo/GAZ_00018546">
        <rdf:type rdf:resource="http://purl.obolibrary.org/obo/ENVO_00000004"/>
        <obo:RO_0001025 rdf:resource="http://purl.obolibrary.org/obo/GAZ_00005251"/>
        <obo:IAO_0000115>A district of Sindh province, Pakistan that was originally part of Larkana District.</obo:IAO_0000115>
        <oboInOwl:hasOBONamespace>GAZ</oboInOwl:hasOBONamespace>
        <oboInOwl:id>GAZ:00018546</oboInOwl:id>
        <rdfs:label>Qamber-Shahdad Kot District</rdfs:label>
    </owl:NamedIndividual>
    


    <!-- http://purl.obolibrary.org/obo/GAZ_00018547 -->

    <owl:NamedIndividual rdf:about="http://purl.obolibrary.org/obo/GAZ_00018547">
        <rdf:type rdf:resource="http://purl.obolibrary.org/obo/ENVO_00000004"/>
        <obo:RO_0001025 rdf:resource="http://purl.obolibrary.org/obo/GAZ_00005251"/>
        <obo:IAO_0000115>A district in the province of Sindh, Pakistan.</obo:IAO_0000115>
        <oboInOwl:hasOBONamespace>GAZ</oboInOwl:hasOBONamespace>
        <oboInOwl:id>GAZ:00018547</oboInOwl:id>
        <rdfs:label>Nawabshah District</rdfs:label>
    </owl:NamedIndividual>
    


    <!-- http://purl.obolibrary.org/obo/GAZ_00018548 -->

    <owl:NamedIndividual rdf:about="http://purl.obolibrary.org/obo/GAZ_00018548">
        <rdf:type rdf:resource="http://purl.obolibrary.org/obo/ENVO_00000004"/>
        <obo:RO_0001025 rdf:resource="http://purl.obolibrary.org/obo/GAZ_00005251"/>
        <obo:IAO_0000115>A district in Sindh Province in Pakistan.</obo:IAO_0000115>
        <oboInOwl:hasOBONamespace>GAZ</oboInOwl:hasOBONamespace>
        <oboInOwl:id>GAZ:00018548</oboInOwl:id>
        <rdfs:label>Sukkur District</rdfs:label>
    </owl:NamedIndividual>
    


    <!-- http://purl.obolibrary.org/obo/GAZ_00018549 -->

    <owl:NamedIndividual rdf:about="http://purl.obolibrary.org/obo/GAZ_00018549">
        <rdf:type rdf:resource="http://purl.obolibrary.org/obo/ENVO_00000004"/>
        <obo:RO_0001025 rdf:resource="http://purl.obolibrary.org/obo/GAZ_00005251"/>
        <obo:IAO_0000115>A district in the Sindh province of Pakistan. Khairpur District is located in northern Sindh and is bounded on the north by Shikarpur and Sukkur, on the east by India. On the south by Sanghar and Nawabshah and on the west by Larkana.</obo:IAO_0000115>
        <oboInOwl:hasOBONamespace>GAZ</oboInOwl:hasOBONamespace>
        <oboInOwl:id>GAZ:00018549</oboInOwl:id>
        <rdfs:label>Khairpur District</rdfs:label>
    </owl:NamedIndividual>
    


    <!-- http://purl.obolibrary.org/obo/GAZ_00018550 -->

    <owl:NamedIndividual rdf:about="http://purl.obolibrary.org/obo/GAZ_00018550">
        <rdf:type rdf:resource="http://purl.obolibrary.org/obo/ENVO_00000004"/>
        <obo:RO_0001025 rdf:resource="http://purl.obolibrary.org/obo/GAZ_00005251"/>
        <obo:IAO_0000115>A district in the Sindh province of Pakistan, the city of Shikarpur is the capital. Shikarpur District borders the districts of Larkana, Jacobabad, Khairpur and Sukkur.</obo:IAO_0000115>
        <oboInOwl:hasOBONamespace>GAZ</oboInOwl:hasOBONamespace>
        <oboInOwl:id>GAZ:00018550</oboInOwl:id>
        <rdfs:label>Shikarpur District</rdfs:label>
    </owl:NamedIndividual>
    


    <!-- http://purl.obolibrary.org/obo/GAZ_00018551 -->

    <owl:NamedIndividual rdf:about="http://purl.obolibrary.org/obo/GAZ_00018551">
        <rdf:type rdf:resource="http://purl.obolibrary.org/obo/ENVO_00000004"/>
        <obo:RO_0001025 rdf:resource="http://purl.obolibrary.org/obo/GAZ_00005251"/>
        <obo:IAO_0000115>A district in the province of Sindh, Pakistan.</obo:IAO_0000115>
        <oboInOwl:hasOBONamespace>GAZ</oboInOwl:hasOBONamespace>
        <oboInOwl:id>GAZ:00018551</oboInOwl:id>
        <rdfs:label>Noushehro Feroz District</rdfs:label>
    </owl:NamedIndividual>
    


    <!-- http://purl.obolibrary.org/obo/GAZ_00018552 -->

    <owl:NamedIndividual rdf:about="http://purl.obolibrary.org/obo/GAZ_00018552">
        <rdf:type rdf:resource="http://purl.obolibrary.org/obo/ENVO_00000004"/>
        <obo:RO_0001025 rdf:resource="http://purl.obolibrary.org/obo/GAZ_00005251"/>
        <obo:IAO_0000115>A district of Sindh Province, Pakistan.</obo:IAO_0000115>
        <oboInOwl:hasOBONamespace>GAZ</oboInOwl:hasOBONamespace>
        <oboInOwl:id>GAZ:00018552</oboInOwl:id>
        <rdfs:label>Dadu District</rdfs:label>
    </owl:NamedIndividual>
    


    <!-- http://purl.obolibrary.org/obo/GAZ_00018553 -->

    <owl:NamedIndividual rdf:about="http://purl.obolibrary.org/obo/GAZ_00018553">
        <rdf:type rdf:resource="http://purl.obolibrary.org/obo/ENVO_00000004"/>
        <obo:RO_0001025 rdf:resource="http://purl.obolibrary.org/obo/GAZ_00005251"/>
        <obo:IAO_0000115>A district of Sindh province of Pakistan.</obo:IAO_0000115>
        <oboInOwl:hasOBONamespace>GAZ</oboInOwl:hasOBONamespace>
        <oboInOwl:id>GAZ:00018553</oboInOwl:id>
        <rdfs:label>Larkana District</rdfs:label>
    </owl:NamedIndividual>
    


    <!-- http://purl.obolibrary.org/obo/GAZ_00018554 -->

    <owl:NamedIndividual rdf:about="http://purl.obolibrary.org/obo/GAZ_00018554">
        <rdf:type rdf:resource="http://purl.obolibrary.org/obo/ENVO_00000004"/>
        <obo:RO_0001025 rdf:resource="http://purl.obolibrary.org/obo/GAZ_00005251"/>
        <obo:IAO_0000115>A district of Sindh Province, Pakistan.</obo:IAO_0000115>
        <oboInOwl:hasOBONamespace>GAZ</oboInOwl:hasOBONamespace>
        <oboInOwl:id>GAZ:00018554</oboInOwl:id>
        <rdfs:label>Ghutki District</rdfs:label>
    </owl:NamedIndividual>
    


    <!-- http://purl.obolibrary.org/obo/GAZ_00018555 -->

    <owl:NamedIndividual rdf:about="http://purl.obolibrary.org/obo/GAZ_00018555">
        <obo:RO_0001025 rdf:resource="http://purl.obolibrary.org/obo/GAZ_00005253"/>
        <obo:IAO_0000115>A tribal area in FATA region of Pakistan. It comprises the area west and southwest of Peshawar between the Tochi River to the north and the Gomal river to the south, forming part of Pakistan&apos;s Federally Administered Tribal Areas (FATA). The North-West Frontier Province lies immediately to the east.</obo:IAO_0000115>
        <oboInOwl:hasOBONamespace>GAZ</oboInOwl:hasOBONamespace>
        <oboInOwl:id>GAZ:00018555</oboInOwl:id>
        <rdfs:label>South Waziristan Agency</rdfs:label>
    </owl:NamedIndividual>
    


    <!-- http://purl.obolibrary.org/obo/GAZ_00018556 -->

    <owl:NamedIndividual rdf:about="http://purl.obolibrary.org/obo/GAZ_00018556">
        <obo:RO_0001025 rdf:resource="http://purl.obolibrary.org/obo/GAZ_00005253"/>
        <obo:IAO_0000115>A tribal area in FATA region of Pakistan. It comprises the area west and south-west of Peshawar between the Tochi river to the north and the Gomal river to the south, forming part of Pakistan&apos;s Federally Administered Tribal Areas (FATA). Miran Shah is capital of North Waziristan. The North-West Frontier Province lies immediately to the east.</obo:IAO_0000115>
        <oboInOwl:hasOBONamespace>GAZ</oboInOwl:hasOBONamespace>
        <oboInOwl:id>GAZ:00018556</oboInOwl:id>
        <rdfs:label>North Waziristan Agency</rdfs:label>
    </owl:NamedIndividual>
    


    <!-- http://purl.obolibrary.org/obo/GAZ_00018557 -->

    <owl:NamedIndividual rdf:about="http://purl.obolibrary.org/obo/GAZ_00018557">
        <obo:RO_0001025 rdf:resource="http://purl.obolibrary.org/obo/GAZ_00018555"/>
        <obo:IAO_0000115>A subdivision of the South Waziristan Agency.</obo:IAO_0000115>
        <oboInOwl:hasOBONamespace>GAZ</oboInOwl:hasOBONamespace>
        <oboInOwl:id>GAZ:00018557</oboInOwl:id>
        <rdfs:label>Sarwakai Subdivision</rdfs:label>
    </owl:NamedIndividual>
    


    <!-- http://purl.obolibrary.org/obo/GAZ_00018558 -->

    <owl:NamedIndividual rdf:about="http://purl.obolibrary.org/obo/GAZ_00018558">
        <obo:RO_0001025 rdf:resource="http://purl.obolibrary.org/obo/GAZ_00018555"/>
        <obo:IAO_0000115>A subdivision of the South Waziristan Agency.</obo:IAO_0000115>
        <oboInOwl:hasOBONamespace>GAZ</oboInOwl:hasOBONamespace>
        <oboInOwl:id>GAZ:00018558</oboInOwl:id>
        <rdfs:label>Wana Subdivision</rdfs:label>
    </owl:NamedIndividual>
    


    <!-- http://purl.obolibrary.org/obo/GAZ_00018559 -->

    <owl:NamedIndividual rdf:about="http://purl.obolibrary.org/obo/GAZ_00018559">
        <obo:RO_0001025 rdf:resource="http://purl.obolibrary.org/obo/GAZ_00018555"/>
        <obo:IAO_0000115>A subdivision of the South Waziristan Agency.</obo:IAO_0000115>
        <oboInOwl:hasOBONamespace>GAZ</oboInOwl:hasOBONamespace>
        <oboInOwl:id>GAZ:00018559</oboInOwl:id>
        <rdfs:label>Ladha Subdivision</rdfs:label>
    </owl:NamedIndividual>
    


    <!-- http://purl.obolibrary.org/obo/GAZ_00018560 -->

    <owl:NamedIndividual rdf:about="http://purl.obolibrary.org/obo/GAZ_00018560">
        <obo:RO_0001025 rdf:resource="http://purl.obolibrary.org/obo/GAZ_00005253"/>
        <obo:IAO_0000115>A tribal agency located in the FATA area of Pakistan. Until the year 2000, when divisions were abolished, Kurram District used to be part of the Peshawar Division of the North-West Frontier Province of Pakistan.</obo:IAO_0000115>
        <oboInOwl:hasOBONamespace>GAZ</oboInOwl:hasOBONamespace>
        <oboInOwl:id>GAZ:00018560</oboInOwl:id>
        <rdfs:label>Kurram Agency</rdfs:label>
    </owl:NamedIndividual>
    


    <!-- http://purl.obolibrary.org/obo/GAZ_00018561 -->

    <owl:NamedIndividual rdf:about="http://purl.obolibrary.org/obo/GAZ_00018561">
        <rdf:type rdf:resource="http://purl.obolibrary.org/obo/ENVO_00000004"/>
        <obo:RO_0001025 rdf:resource="http://purl.obolibrary.org/obo/GAZ_00005253"/>
        <obo:IAO_0000115>An Agency (district) of the Federally Administered Tribal Areas (FATA) of Pakistan.</obo:IAO_0000115>
        <oboInOwl:hasOBONamespace>GAZ</oboInOwl:hasOBONamespace>
        <oboInOwl:id>GAZ:00018561</oboInOwl:id>
        <rdfs:label>Bajaur Agency</rdfs:label>
    </owl:NamedIndividual>
    


    <!-- http://purl.obolibrary.org/obo/GAZ_00018562 -->

    <owl:NamedIndividual rdf:about="http://purl.obolibrary.org/obo/GAZ_00018562">
        <obo:RO_0001025 rdf:resource="http://purl.obolibrary.org/obo/GAZ_00005253"/>
        <obo:IAO_0000115>A tribal area in FATA region of Pakistan.</obo:IAO_0000115>
        <oboInOwl:hasOBONamespace>GAZ</oboInOwl:hasOBONamespace>
        <oboInOwl:id>GAZ:00018562</oboInOwl:id>
        <rdfs:label>Khyber Agency</rdfs:label>
    </owl:NamedIndividual>
    


    <!-- http://purl.obolibrary.org/obo/GAZ_00018563 -->

    <owl:NamedIndividual rdf:about="http://purl.obolibrary.org/obo/GAZ_00018563">
        <obo:RO_0001025 rdf:resource="http://purl.obolibrary.org/obo/GAZ_00005253"/>
        <obo:IAO_0000115>One of the Federally Administered Tribal Areas of Pakistan. It is bounded by Kurram Agency in the west, Khyber in the north, Kohat District on the south and Peshawar in the east.</obo:IAO_0000115>
        <oboInOwl:hasOBONamespace>GAZ</oboInOwl:hasOBONamespace>
        <oboInOwl:id>GAZ:00018563</oboInOwl:id>
        <rdfs:label>Orakzai Agency</rdfs:label>
    </owl:NamedIndividual>
    


    <!-- http://purl.obolibrary.org/obo/GAZ_00018564 -->

    <owl:NamedIndividual rdf:about="http://purl.obolibrary.org/obo/GAZ_00018564">
        <obo:RO_0001025 rdf:resource="http://purl.obolibrary.org/obo/GAZ_00005253"/>
        <obo:IAO_0000115>A tribal area in FATA region of Pakistan. The agency was created in 1951 before which the Mohmand Tribes were administered by the Deputy Commissioner based in Peshawar, North-West Frontier Province, Pakistan.</obo:IAO_0000115>
        <oboInOwl:hasOBONamespace>GAZ</oboInOwl:hasOBONamespace>
        <oboInOwl:id>GAZ:00018564</oboInOwl:id>
        <rdfs:label>Mohmand Agency</rdfs:label>
    </owl:NamedIndividual>
    


    <!-- http://purl.obolibrary.org/obo/GAZ_00018565 -->

    <owl:NamedIndividual rdf:about="http://purl.obolibrary.org/obo/GAZ_00018565">
        <rdf:type rdf:resource="http://purl.obolibrary.org/obo/ENVO_00000004"/>
        <obo:RO_0001025 rdf:resource="http://purl.obolibrary.org/obo/GAZ_00005257"/>
        <obo:IAO_0000115>An administrative division of Azad Kashmir.</obo:IAO_0000115>
        <oboInOwl:hasOBONamespace>GAZ</oboInOwl:hasOBONamespace>
        <oboInOwl:id>GAZ:00018565</oboInOwl:id>
        <rdfs:label>Muzaffarabad Division</rdfs:label>
    </owl:NamedIndividual>
    


    <!-- http://purl.obolibrary.org/obo/GAZ_00018566 -->

    <owl:NamedIndividual rdf:about="http://purl.obolibrary.org/obo/GAZ_00018566">
        <rdf:type rdf:resource="http://purl.obolibrary.org/obo/ENVO_00000004"/>
        <obo:RO_0001025 rdf:resource="http://purl.obolibrary.org/obo/GAZ_00005257"/>
        <obo:IAO_0000115>An administrative division of Azad Kashmir.</obo:IAO_0000115>
        <oboInOwl:hasOBONamespace>GAZ</oboInOwl:hasOBONamespace>
        <oboInOwl:id>GAZ:00018566</oboInOwl:id>
        <rdfs:label>Mirpur Division</rdfs:label>
    </owl:NamedIndividual>
    


    <!-- http://purl.obolibrary.org/obo/GAZ_00018567 -->

    <owl:NamedIndividual rdf:about="http://purl.obolibrary.org/obo/GAZ_00018567">
        <rdf:type rdf:resource="http://purl.obolibrary.org/obo/ENVO_00000004"/>
        <obo:RO_0001025 rdf:resource="http://purl.obolibrary.org/obo/GAZ_00018566"/>
        <obo:IAO_0000115>A district of Azad Kashmir, which is the Pakistani-administered part of the former princely State of Jammu and Kashmir. The area now comprising district Kotli was a sub-division of Mirpur District up to the year 1975. Prior to 1947, it was a part of the Jammu area. The district is bounded by the Indian State of Jammu and Kashmir in the east, and by Mirpur District in the south and Rawalakot to its north.</obo:IAO_0000115>
        <oboInOwl:hasOBONamespace>GAZ</oboInOwl:hasOBONamespace>
        <oboInOwl:id>GAZ:00018567</oboInOwl:id>
        <rdfs:label>Kotli District</rdfs:label>
    </owl:NamedIndividual>
    


    <!-- http://purl.obolibrary.org/obo/GAZ_00018568 -->

    <owl:NamedIndividual rdf:about="http://purl.obolibrary.org/obo/GAZ_00018568">
        <rdf:type rdf:resource="http://purl.obolibrary.org/obo/ENVO_00000004"/>
        <obo:RO_0001025 rdf:resource="http://purl.obolibrary.org/obo/GAZ_00018566"/>
        <obo:IAO_0000115>A district in Pakistan&apos;s Azad Kashmir Territory.</obo:IAO_0000115>
        <oboInOwl:hasOBONamespace>GAZ</oboInOwl:hasOBONamespace>
        <oboInOwl:id>GAZ:00018568</oboInOwl:id>
        <rdfs:label>Mirpur District</rdfs:label>
    </owl:NamedIndividual>
    


    <!-- http://purl.obolibrary.org/obo/GAZ_00018569 -->

    <owl:NamedIndividual rdf:about="http://purl.obolibrary.org/obo/GAZ_00018569">
        <obo:RO_0001025 rdf:resource="http://purl.obolibrary.org/obo/GAZ_00018566"/>
        <obo:IAO_0000115>The southernmost of the eight districts of Azad Kashmir. The district is bounded by Mirpur district to the northwest (and is 50 km from Mirpur city), and Punjab province in the west and south. It also shares borders with Indian administered Kashmir to the east.</obo:IAO_0000115>
        <oboInOwl:hasOBONamespace>GAZ</oboInOwl:hasOBONamespace>
        <oboInOwl:id>GAZ:00018569</oboInOwl:id>
        <rdfs:label>Bhimber District</rdfs:label>
    </owl:NamedIndividual>
    


    <!-- http://purl.obolibrary.org/obo/GAZ_00018570 -->

    <owl:NamedIndividual rdf:about="http://purl.obolibrary.org/obo/GAZ_00018570">
        <obo:RO_0001025 rdf:resource="http://purl.obolibrary.org/obo/GAZ_00018565"/>
        <obo:IAO_0000115>One of the eight districts of Azad Kashmir (the area of Kashmir administered by Pakistan).</obo:IAO_0000115>
        <oboInOwl:hasOBONamespace>GAZ</oboInOwl:hasOBONamespace>
        <oboInOwl:id>GAZ:00018570</oboInOwl:id>
        <rdfs:label>Poonch District</rdfs:label>
    </owl:NamedIndividual>
    


    <!-- http://purl.obolibrary.org/obo/GAZ_00018571 -->

    <owl:NamedIndividual rdf:about="http://purl.obolibrary.org/obo/GAZ_00018571">
        <rdf:type rdf:resource="http://purl.obolibrary.org/obo/ENVO_00000004"/>
        <obo:RO_0001025 rdf:resource="http://purl.obolibrary.org/obo/GAZ_00018565"/>
        <obo:IAO_0000115>A district of Azad Kashmir in Pakistan.</obo:IAO_0000115>
        <oboInOwl:hasOBONamespace>GAZ</oboInOwl:hasOBONamespace>
        <oboInOwl:id>GAZ:00018571</oboInOwl:id>
        <rdfs:label>Sudhnati District</rdfs:label>
    </owl:NamedIndividual>
    


    <!-- http://purl.obolibrary.org/obo/GAZ_00018572 -->

    <owl:NamedIndividual rdf:about="http://purl.obolibrary.org/obo/GAZ_00018572">
        <obo:RO_0001025 rdf:resource="http://purl.obolibrary.org/obo/GAZ_00018565"/>
        <obo:IAO_0000115>One of the eight districts of Azad Kashmir, Pakistan.</obo:IAO_0000115>
        <oboInOwl:hasOBONamespace>GAZ</oboInOwl:hasOBONamespace>
        <oboInOwl:id>GAZ:00018572</oboInOwl:id>
        <rdfs:label>Muzaffarabad District</rdfs:label>
    </owl:NamedIndividual>
    


    <!-- http://purl.obolibrary.org/obo/GAZ_00018573 -->

    <owl:NamedIndividual rdf:about="http://purl.obolibrary.org/obo/GAZ_00018573">
        <obo:RO_0001025 rdf:resource="http://purl.obolibrary.org/obo/GAZ_00018565"/>
        <obo:IAO_0000115>One of the eight districts of Azad Kashmir, Pakistan. Until recently it was part of Muzaffarabad District. It is bounded by the Gilgit (Northern Areas) to the North, with Kupwara and Baramulla Districts of J&amp;k, India to the South and Southeast, Muzaffarabad District to the Southwest and Mansehra District to the West.</obo:IAO_0000115>
        <oboInOwl:hasOBONamespace>GAZ</oboInOwl:hasOBONamespace>
        <oboInOwl:id>GAZ:00018573</oboInOwl:id>
        <rdfs:label>Neelum District</rdfs:label>
    </owl:NamedIndividual>
    


    <!-- http://purl.obolibrary.org/obo/GAZ_00018574 -->

    <owl:NamedIndividual rdf:about="http://purl.obolibrary.org/obo/GAZ_00018574">
        <obo:RO_0001025 rdf:resource="http://purl.obolibrary.org/obo/GAZ_00018565"/>
        <obo:IAO_0000115>One of the eight districts of Azad Kashmir, Pakistan. The district, which had been part of Poonch District, was created in 1988[1]. The district is bounded by Muzaffarabad District to the north, with Poonch district to the south, and with Poonch District of the Indian-administered Jammu and Kashmir to the east and is bounded to Punjab (Pakistan) in the west.</obo:IAO_0000115>
        <oboInOwl:hasOBONamespace>GAZ</oboInOwl:hasOBONamespace>
        <oboInOwl:id>GAZ:00018574</oboInOwl:id>
        <rdfs:label>Bagh District</rdfs:label>
    </owl:NamedIndividual>
    


    <!-- http://purl.obolibrary.org/obo/GAZ_00018575 -->

    <owl:NamedIndividual rdf:about="http://purl.obolibrary.org/obo/GAZ_00018575">
        <obo:RO_0001025 rdf:resource="http://purl.obolibrary.org/obo/GAZ_00005256"/>
        <obo:IAO_0000115>A division of the Federally Administered Northern Areas.</obo:IAO_0000115>
        <oboInOwl:hasOBONamespace>GAZ</oboInOwl:hasOBONamespace>
        <oboInOwl:id>GAZ:00018575</oboInOwl:id>
        <rdfs:label>Gilgit Division</rdfs:label>
    </owl:NamedIndividual>
    


    <!-- http://purl.obolibrary.org/obo/GAZ_00018576 -->

    <owl:NamedIndividual rdf:about="http://purl.obolibrary.org/obo/GAZ_00018576">
        <obo:RO_0001025 rdf:resource="http://purl.obolibrary.org/obo/GAZ_00018575"/>
        <obo:IAO_0000115>The northernmost part of the Northern Areas of Pakistan. Ghizer is also a contact point between Gilgit and Chitral (which are connected via Shandur Pass). It joins with Wakhan strip on its north-west, and China on its northern borders. On its west, there is Chitral District of NWFP; and on its east is situated Gilgit. Diamer District is on its south, which is again a part of the Northern areas. Gakuch is the capital of the Ghizer District.</obo:IAO_0000115>
        <oboInOwl:hasOBONamespace>GAZ</oboInOwl:hasOBONamespace>
        <oboInOwl:id>GAZ:00018576</oboInOwl:id>
        <rdfs:label>Ghizer District</rdfs:label>
    </owl:NamedIndividual>
    


    <!-- http://purl.obolibrary.org/obo/GAZ_00018578 -->

    <owl:NamedIndividual rdf:about="http://purl.obolibrary.org/obo/GAZ_00018578">
        <obo:RO_0001025 rdf:resource="http://purl.obolibrary.org/obo/GAZ_00018575"/>
        <obo:IAO_0000115>One of the six districts of the Northern Areas of Pakistan. The district contains the Astore Valley and is bounded to the east by Diamer District (from which is was separated in 2004), to the north by Gilgit District, to the east by Skardu District and to the south by Azad Kashmir and the North-West Frontier Province.</obo:IAO_0000115>
        <oboInOwl:hasOBONamespace>GAZ</oboInOwl:hasOBONamespace>
        <oboInOwl:id>GAZ:00018578</oboInOwl:id>
        <rdfs:label>Astore District</rdfs:label>
    </owl:NamedIndividual>
    


    <!-- http://purl.obolibrary.org/obo/GAZ_00018579 -->

    <owl:NamedIndividual rdf:about="http://purl.obolibrary.org/obo/GAZ_00018579">
        <obo:RO_0001025 rdf:resource="http://purl.obolibrary.org/obo/GAZ_00005256"/>
        <obo:IAO_0000115>A division of the Federally Administered Northern Areas.</obo:IAO_0000115>
        <oboInOwl:hasOBONamespace>GAZ</oboInOwl:hasOBONamespace>
        <oboInOwl:id>GAZ:00018579</oboInOwl:id>
        <rdfs:label>Baltistan Division</rdfs:label>
    </owl:NamedIndividual>
    


    <!-- http://purl.obolibrary.org/obo/GAZ_00018580 -->

    <owl:NamedIndividual rdf:about="http://purl.obolibrary.org/obo/GAZ_00018580">
        <obo:RO_0001025 rdf:resource="http://purl.obolibrary.org/obo/GAZ_00018579"/>
        <obo:IAO_0000115>One of the six districts of Northern Areas of Pakistan. It is bounded on the east by Ghanche District, on the northeast by Xinjiang, (China), on the south by Baramulla and Kargil District, on the west by district Astore and on the north by Gilgit District.</obo:IAO_0000115>
        <oboInOwl:hasOBONamespace>GAZ</oboInOwl:hasOBONamespace>
        <oboInOwl:id>GAZ:00018580</oboInOwl:id>
        <rdfs:label>Skardu District</rdfs:label>
    </owl:NamedIndividual>
    


    <!-- http://purl.obolibrary.org/obo/GAZ_00018581 -->

    <owl:NamedIndividual rdf:about="http://purl.obolibrary.org/obo/GAZ_00018581">
        <obo:RO_0001025 rdf:resource="http://purl.obolibrary.org/obo/GAZ_00018579"/>
        <obo:IAO_0000115>The easternmost district of the Northern Areas, Pakistan. To its northeast is Xinjiang (China), to the north and northwest is Skardu District, to its west is Astore District and to its south is Ladakh District in the Indian State of Jammu and Kashmir.</obo:IAO_0000115>
        <oboInOwl:hasOBONamespace>GAZ</oboInOwl:hasOBONamespace>
        <oboInOwl:id>GAZ:00018581</oboInOwl:id>
        <rdfs:label>Ghanche District</rdfs:label>
    </owl:NamedIndividual>
    


    <!-- http://purl.obolibrary.org/obo/GAZ_00018582 -->

    <owl:NamedIndividual rdf:about="http://purl.obolibrary.org/obo/GAZ_00018582">
        <rdf:type rdf:resource="http://purl.obolibrary.org/obo/ENVO_00000004"/>
        <obo:RO_0001025 rdf:resource="http://purl.obolibrary.org/obo/GAZ_00018575"/>
        <obo:IAO_0000115>A district of the Pakistani Northern Areas and is the district in which the Karakoram Highway enters that territory from Pakistan&apos;s NWFP. The capital of the Diamir District is Chilas. The Diamir District is bounded by the Astore District in the east, Pakistan&apos;s NWFP in the southwest (separated by the Babusar Pass or Babusar Top), Neelum District of Azad Kashmir in the south, the Ghizar District in the north and northwest, and the Gilgit District in the north and northeast.</obo:IAO_0000115>
        <oboInOwl:hasOBONamespace>GAZ</oboInOwl:hasOBONamespace>
        <oboInOwl:id>GAZ:00018582</oboInOwl:id>
        <rdfs:label>Diamer District</rdfs:label>
    </owl:NamedIndividual>
    


    <!-- http://purl.obolibrary.org/obo/GAZ_00018583 -->

    <owl:NamedIndividual rdf:about="http://purl.obolibrary.org/obo/GAZ_00018583">
        <rdf:type rdf:resource="http://purl.obolibrary.org/obo/ENVO_00000004"/>
        <obo:RO_0001025 rdf:resource="http://purl.obolibrary.org/obo/GAZ_00018575"/>
        <obo:IAO_0000115>A district bounded by Wakhan Corridor (Afghanistan) in the north, Xinjiang (China) in the north / northeast, Skardu District in the south / southeast. The town of Gilgit is the capital of Gilgit District.</obo:IAO_0000115>
        <oboInOwl:hasOBONamespace>GAZ</oboInOwl:hasOBONamespace>
        <oboInOwl:id>GAZ:00018583</oboInOwl:id>
        <rdfs:label>Gilgit District</rdfs:label>
    </owl:NamedIndividual>
    


    <!-- http://purl.obolibrary.org/obo/GAZ_00055997 -->

    <owl:NamedIndividual rdf:about="http://purl.obolibrary.org/obo/GAZ_00055997">
        <obo:RO_0001025 rdf:resource="http://purl.obolibrary.org/obo/GAZ_00005246"/>
        <obo:IAO_0000115>A mountain range in Pakistan and one of the bordering ranges between the Iranian Plateau and the Indian subcontinent. Bordering the Sulaiman Range to the north are the arid highlands of the Hindu Kush, with more than 50 percent of the lands there lying above 2,000 m. The highest peak of Sulaiman Mountains is Takht-e-Sulaiman (3,487 m) in Balochistan, Pakistan.</obo:IAO_0000115>
        <oboInOwl:hasOBONamespace>GAZ</oboInOwl:hasOBONamespace>
        <oboInOwl:id>GAZ:00055997</oboInOwl:id>
        <rdfs:label>Sulaiman Mountains</rdfs:label>
    </owl:NamedIndividual>
    


    <!-- http://purl.obolibrary.org/obo/GAZ_00055998 -->

    <owl:NamedIndividual rdf:about="http://purl.obolibrary.org/obo/GAZ_00055998">
        <obo:RO_0001025 rdf:resource="http://purl.obolibrary.org/obo/GAZ_00005248"/>
        <obo:IAO_0000115>A mud volcano.</obo:IAO_0000115>
        <oboInOwl:hasOBONamespace>GAZ</oboInOwl:hasOBONamespace>
        <oboInOwl:id>GAZ:00055998</oboInOwl:id>
        <rdfs:label>Jebel e Ghurab Ud Volcano</rdfs:label>
    </owl:NamedIndividual>
    


    <!-- http://purl.obolibrary.org/obo/GAZ_00055999 -->

    <owl:NamedIndividual rdf:about="http://purl.obolibrary.org/obo/GAZ_00055999">
        <obo:RO_0001025 rdf:resource="http://purl.obolibrary.org/obo/GAZ_00005248"/>
        <obo:IAO_0000115>A mud volcano.</obo:IAO_0000115>
        <oboInOwl:hasOBONamespace>GAZ</oboInOwl:hasOBONamespace>
        <oboInOwl:id>GAZ:00055999</oboInOwl:id>
        <rdfs:label>Chandragup Mud Volcano</rdfs:label>
    </owl:NamedIndividual>
    


    <!-- http://purl.obolibrary.org/obo/GAZ_00056000 -->

    <owl:NamedIndividual rdf:about="http://purl.obolibrary.org/obo/GAZ_00056000">
        <obo:RO_0001025 rdf:resource="http://purl.obolibrary.org/obo/GAZ_00005248"/>
        <obo:IAO_0000115>A mud volcano.</obo:IAO_0000115>
        <oboInOwl:hasOBONamespace>GAZ</oboInOwl:hasOBONamespace>
        <oboInOwl:id>GAZ:00056000</oboInOwl:id>
        <rdfs:label>Hingol Mud Volcano</rdfs:label>
    </owl:NamedIndividual>
    


    <!-- http://purl.obolibrary.org/obo/GAZ_00056899 -->

    <owl:NamedIndividual rdf:about="http://purl.obolibrary.org/obo/GAZ_00056899">
        <obo:RO_0001025 rdf:resource="http://purl.obolibrary.org/obo/GAZ_00005246"/>
        <obo:IAO_0000115>A mountain range that is located in Balochistan and Sindh provinces of Pakistan. It extends southward for about (300 km from the Mula River in east-central Balochistan to Cape Muari (Monze) west of Karachi on the Arabian Sea. The range forms the boundary between the Lower Indus Plain (east) and southern Balochistan (west). It consists of a series of parallel, rock hill ridges rising from 1,200 m in the south to nearly 2,500 m in the north. It is drained in the north by the Kolachi River and in the south by the Hub River and Lyari River, which flow to the Arabian Sea.</obo:IAO_0000115>
        <oboInOwl:hasOBONamespace>GAZ</oboInOwl:hasOBONamespace>
        <oboInOwl:id>GAZ:00056899</oboInOwl:id>
        <rdfs:label>Kirthar Mountains</rdfs:label>
    </owl:NamedIndividual>
    


    <!-- http://purl.obolibrary.org/obo/GAZ_00056900 -->

    <owl:NamedIndividual rdf:about="http://purl.obolibrary.org/obo/GAZ_00056900">
        <obo:RO_0001025 rdf:resource="http://purl.obolibrary.org/obo/GAZ_00018552"/>
        <obo:RO_0001025 rdf:resource="http://purl.obolibrary.org/obo/GAZ_00056899"/>
        <obo:RO_0001025 rdf:resource="http://purl.obolibrary.org/obo/GAZ_00400093"/>
        <obo:IAO_0000115>A national park located in Kirthar Mountains range.</obo:IAO_0000115>
        <oboInOwl:hasOBONamespace>GAZ</oboInOwl:hasOBONamespace>
        <oboInOwl:id>GAZ:00056900</oboInOwl:id>
        <rdfs:label>Kirthar National Park</rdfs:label>
    </owl:NamedIndividual>
    


    <!-- http://purl.obolibrary.org/obo/GAZ_00056902 -->

    <owl:NamedIndividual rdf:about="http://purl.obolibrary.org/obo/GAZ_00056902">
        <obo:IAO_0000115>A mountain range in Afghanistan as well as in the North-West Frontier Province and Northern Areas of Pakistan. It is the westernmost extension of the Pamir Mountains, the Karakoram Range, and the Himalayas.</obo:IAO_0000115>
        <oboInOwl:hasOBONamespace>GAZ</oboInOwl:hasOBONamespace>
        <oboInOwl:id>GAZ:00056902</oboInOwl:id>
        <rdfs:label>Hindu Kush</rdfs:label>
    </owl:NamedIndividual>
    


    <!-- http://purl.obolibrary.org/obo/GAZ_00056903 -->

    <owl:NamedIndividual rdf:about="http://purl.obolibrary.org/obo/GAZ_00056903">
        <rdf:type rdf:resource="http://purl.obolibrary.org/obo/ENVO_00000104"/>
        <rdf:type rdf:resource="http://purl.obolibrary.org/obo/ENVO_00000106"/>
        <obo:RO_0001025 rdf:resource="http://purl.obolibrary.org/obo/GAZ_00005246"/>
        <obo:IAO_0000115>A range of mountains on the Pakistan-Afghanistan border, up to 15,620ft (4,761 m) above sea-level at Mount Sikaram, straight and rigid, towering above all surrounding hills, it is near the Kabul River. A spur of the range is crossed by the Khyber Pass.</obo:IAO_0000115>
        <oboInOwl:hasOBONamespace>GAZ</oboInOwl:hasOBONamespace>
        <oboInOwl:id>GAZ:00056903</oboInOwl:id>
        <rdfs:label>Safed Koh Mountains</rdfs:label>
    </owl:NamedIndividual>
    


    <!-- http://purl.obolibrary.org/obo/GAZ_00056904 -->

    <owl:NamedIndividual rdf:about="http://purl.obolibrary.org/obo/GAZ_00056904">
        <obo:RO_0001025 rdf:resource="http://purl.obolibrary.org/obo/GAZ_00005249"/>
        <obo:IAO_0000115>A hill system in the Punjab province of Pakistan, deriving its name from its extensive deposits of rock salt. The range extends from the Jhelum River to the Indus, across the northern portion of the Punjab province.</obo:IAO_0000115>
        <oboInOwl:hasOBONamespace>GAZ</oboInOwl:hasOBONamespace>
        <oboInOwl:id>GAZ:00056904</oboInOwl:id>
        <rdfs:label>Salt Range</rdfs:label>
    </owl:NamedIndividual>
    


    <!-- http://purl.obolibrary.org/obo/GAZ_00056905 -->

    <owl:NamedIndividual rdf:about="http://purl.obolibrary.org/obo/GAZ_00056905">
        <obo:RO_0001025 rdf:resource="http://purl.obolibrary.org/obo/GAZ_00005248"/>
        <obo:IAO_0000115>A Southern offshoot of the Himalayas in the Balochistan region of Pakistan.</obo:IAO_0000115>
        <oboInOwl:hasOBONamespace>GAZ</oboInOwl:hasOBONamespace>
        <oboInOwl:id>GAZ:00056905</oboInOwl:id>
        <rdfs:label>Toba Kakar Range</rdfs:label>
    </owl:NamedIndividual>
    


    <!-- http://purl.obolibrary.org/obo/GAZ_00056906 -->

    <owl:NamedIndividual rdf:about="http://purl.obolibrary.org/obo/GAZ_00056906">
        <obo:RO_0001025 rdf:resource="http://purl.obolibrary.org/obo/GAZ_00018575"/>
        <obo:IAO_0000115>A subrange of the Karakoram range. They are located in the Gilgit District of the Northern Areas of Pakistan. They are bordered on the north by Barpu and Chogo Lungma Glaciers; on the east by the Shigar River; on the south by the Gilgit and Indus Rivers, and on the west by the Hunza River.</obo:IAO_0000115>
        <oboInOwl:hasOBONamespace>GAZ</oboInOwl:hasOBONamespace>
        <oboInOwl:id>GAZ:00056906</oboInOwl:id>
        <rdfs:label>Rakaposhi-Haramosh Mountains</rdfs:label>
    </owl:NamedIndividual>
    


    <!-- http://purl.obolibrary.org/obo/GAZ_00056907 -->

    <owl:NamedIndividual rdf:about="http://purl.obolibrary.org/obo/GAZ_00056907">
        <obo:RO_0001025 rdf:resource="http://purl.obolibrary.org/obo/GAZ_00005256"/>
        <obo:IAO_0000115>A subrange of the Karakoram range in the Northern Areas of Pakistan. The Spantik-Sosbun Mountains are a narrow range, about 120 km long, trending roughly east-west. On the north, the range is bounded by the important Hispar and Biafo Glaciers, across which lie the Hispar Muztagh and Panmah Muztagh respectively. On the southwest, the Barpu Glacier and the longer Chogo Lungma Glacier separate the range from the Rakaposhi-Haramosh Mountains; the pass known as the Polan La (5840 m) separates the Barpu from the Chogo Lungma, and links the two ranges. On the southeast, the Braldu River separates the range from the somewhat lower Mango Gusor Mountains.</obo:IAO_0000115>
        <oboInOwl:hasOBONamespace>GAZ</oboInOwl:hasOBONamespace>
        <oboInOwl:id>GAZ:00056907</oboInOwl:id>
        <rdfs:label>Spantik-Sosbun Mountains</rdfs:label>
    </owl:NamedIndividual>
    


    <!-- http://purl.obolibrary.org/obo/GAZ_00056908 -->

    <owl:NamedIndividual rdf:about="http://purl.obolibrary.org/obo/GAZ_00056908">
        <obo:RO_0001025 rdf:resource="http://purl.obolibrary.org/obo/GAZ_00018575"/>
        <obo:IAO_0000115>A sub-range of the Karakoram mountain range. It is located in the Gilgit District of the Northern Areas of Pakistan, west of the Hunza Valley. It is the westernmost sub-range of the Karakoram; it runs from Chalt village, in Bar valley, on the east, to Kampir Dior in the Kurumbar valley, which separates the Pamir and Hindu Kush ranges from the Karakoram.</obo:IAO_0000115>
        <oboInOwl:hasOBONamespace>GAZ</oboInOwl:hasOBONamespace>
        <oboInOwl:id>GAZ:00056908</oboInOwl:id>
        <rdfs:label>Batura Muztagh</rdfs:label>
    </owl:NamedIndividual>
    


    <!-- http://purl.obolibrary.org/obo/GAZ_00056909 -->

    <owl:NamedIndividual rdf:about="http://purl.obolibrary.org/obo/GAZ_00056909">
        <obo:RO_0001025 rdf:resource="http://purl.obolibrary.org/obo/GAZ_00056919"/>
        <obo:IAO_0000115>A sub-range of the Karakoram mountain range. It is located in the Gojal region of the Northern Areas of Pakistan, north of Hispar Glacier, south of Shimshal Valley, and east of the Hunza Valley.</obo:IAO_0000115>
        <oboInOwl:hasOBONamespace>GAZ</oboInOwl:hasOBONamespace>
        <oboInOwl:id>GAZ:00056909</oboInOwl:id>
        <rdfs:label>Hispar Muztagh</rdfs:label>
    </owl:NamedIndividual>
    


    <!-- http://purl.obolibrary.org/obo/GAZ_00056910 -->

    <owl:NamedIndividual rdf:about="http://purl.obolibrary.org/obo/GAZ_00056910">
        <obo:RO_0001025 rdf:resource="http://purl.obolibrary.org/obo/GAZ_00005256"/>
        <obo:IAO_0000115>A subrange of the Karakoram range in the Northern Areas of Pakistan. On the south, the range is separated from the Hispar Muztagh by the valley of the Shimshal River. On the north, the range is dilineated from the North Ghujerab Mountains by the Ghujerab River; the combined range is bounded on the north by the Khunjerab River, along which lies the Karakoram Highway leading to Khunjerab Pass. On the west, the South Ghujerab Mountains are bounded by the Hunza River and its tributary, the lower Khunjerab River.</obo:IAO_0000115>
        <oboInOwl:hasOBONamespace>GAZ</oboInOwl:hasOBONamespace>
        <oboInOwl:id>GAZ:00056910</oboInOwl:id>
        <rdfs:label>South Ghujerab Mountains</rdfs:label>
    </owl:NamedIndividual>
    


    <!-- http://purl.obolibrary.org/obo/GAZ_00056911 -->

    <owl:NamedIndividual rdf:about="http://purl.obolibrary.org/obo/GAZ_00056911">
        <obo:RO_0001025 rdf:resource="http://purl.obolibrary.org/obo/GAZ_00018579"/>
        <obo:IAO_0000115>A subrange of the Karakoram range, in Baltistan, a district of the Northern Areas of Pakistan. The Panmah Muztagh lies in the heart of the Karakoram, northwest of the Baltoro Muztagh (home of the eight thousand meter peaks of the Karakoram), and southeast of the Hispar Muztagh. On the southwest, it is separated from the Spantik-Sosbun Mountains by the Biafo Glacier. The Skamri Glacier and the Braldu Glacier separate it from the Wesm Mountains to the north. The Panmah, Nobande Sande, Choktoi, and Chiring Glaciers lie within the range.</obo:IAO_0000115>
        <oboInOwl:hasOBONamespace>GAZ</oboInOwl:hasOBONamespace>
        <oboInOwl:id>GAZ:00056911</oboInOwl:id>
        <rdfs:label>Panmah Muztagh</rdfs:label>
    </owl:NamedIndividual>
    


    <!-- http://purl.obolibrary.org/obo/GAZ_00056912 -->

    <owl:NamedIndividual rdf:about="http://purl.obolibrary.org/obo/GAZ_00056912">
        <obo:IAO_0000115>A Chinese subrange of the Karakoram mountain range. It lies north of the Baltoro Muztagh.</obo:IAO_0000115>
        <oboInOwl:hasOBONamespace>GAZ</oboInOwl:hasOBONamespace>
        <oboInOwl:id>GAZ:00056912</oboInOwl:id>
        <rdfs:label>Yengisogat</rdfs:label>
    </owl:NamedIndividual>
    


    <!-- http://purl.obolibrary.org/obo/GAZ_00056913 -->

    <owl:NamedIndividual rdf:about="http://purl.obolibrary.org/obo/GAZ_00056913">
        <obo:RO_0001025 rdf:resource="http://purl.obolibrary.org/obo/GAZ_00018579"/>
        <obo:IAO_0000115>A subrange of the Karakoram mountain range. It is located on the north and east sides of the Baltoro Glacier, in Baltistan, part of the Northern Areas of Pakistan; and in Xinjiang, China. The crest of the range forms part of the Pakistan-China border.</obo:IAO_0000115>
        <oboInOwl:hasOBONamespace>GAZ</oboInOwl:hasOBONamespace>
        <oboInOwl:id>GAZ:00056913</oboInOwl:id>
        <rdfs:label>Baltoro Muztagh</rdfs:label>
    </owl:NamedIndividual>
    


    <!-- http://purl.obolibrary.org/obo/GAZ_00056914 -->

    <owl:NamedIndividual rdf:about="http://purl.obolibrary.org/obo/GAZ_00056914">
        <obo:RO_0001025 rdf:resource="http://purl.obolibrary.org/obo/GAZ_00005256"/>
        <obo:IAO_0000115>A subrange of the Karakoram range. They are located in the heart of the Karakoram, on the southwest side of the Siachen Glacier, one of the longest glaciers outside of the polar regions. They span the disputed border between the Northern Areas of Pakistan and the Kashmir region of India. On the southwest side, the Saltoro Mountains drop steeply to the valleys of the Kondus and Dansam Rivers, which join to form the Saltoro River, a tributary of the Shyok River. This in turn flows into the Indus River. To the northwest, the Kondus Glacier separates the range from the neighboring Masherbrum Mountains, while on the southeast, the Gyong River, Glacier, and Pass (Gyong La) separate the range from the Kailas Mountains.</obo:IAO_0000115>
        <oboInOwl:hasOBONamespace>GAZ</oboInOwl:hasOBONamespace>
        <oboInOwl:id>GAZ:00056914</oboInOwl:id>
        <rdfs:label>Saltoro Mountains</rdfs:label>
    </owl:NamedIndividual>
    


    <!-- http://purl.obolibrary.org/obo/GAZ_00056915 -->

    <owl:NamedIndividual rdf:about="http://purl.obolibrary.org/obo/GAZ_00056915">
        <obo:RO_0001025 rdf:resource="http://purl.obolibrary.org/obo/GAZ_00018579"/>
        <obo:IAO_0000115>A subrange of the Karakoram range. They are located on the south side of the Baltoro Glacier, in Baltistan, part of the Northern Areas of Pakistan. The southern side of the range is drained by the Hushe River.</obo:IAO_0000115>
        <oboInOwl:hasOBONamespace>GAZ</oboInOwl:hasOBONamespace>
        <oboInOwl:id>GAZ:00056915</oboInOwl:id>
        <rdfs:label>Masherbrum Mountains</rdfs:label>
    </owl:NamedIndividual>
    


    <!-- http://purl.obolibrary.org/obo/GAZ_00056916 -->

    <owl:NamedIndividual rdf:about="http://purl.obolibrary.org/obo/GAZ_00056916">
        <obo:IAO_0000115>A remote subrange of the Karakoram range divided between India and Pakistan along the disputed line of control of Northern Areas of Pakistan, Jammu and Kashmir State of India and Xinjiang, China. It lies just north of the Siachen Glacier, one of the longest glaciers outside of the polar regions.</obo:IAO_0000115>
        <oboInOwl:hasOBONamespace>GAZ</oboInOwl:hasOBONamespace>
        <oboInOwl:id>GAZ:00056916</oboInOwl:id>
        <rdfs:label>Siachen Muztagh</rdfs:label>
    </owl:NamedIndividual>
    


    <!-- http://purl.obolibrary.org/obo/GAZ_00056917 -->

    <owl:NamedIndividual rdf:about="http://purl.obolibrary.org/obo/GAZ_00056917">
        <obo:IAO_0000115>One of the most remote subranges of the Karakoram range, in far northwestern India, near the disputed border with Pakistan. The Rimo Muztagh is bordered on the north by the Rimo Glacier, which drains to the east into the upper Shyok River, and by the Teram Shehr Glacier, a tributary of the Siachen Glacier. To the northeast lie the Northeast Rimo Mountains and the Karakoram Pass, a pass on one of the historically important trade routes into Central Asia. To the north lies the eastern end of the Siachen Muztagh. On the east side of the range, the upper Shyok River divides it from the Depsang Plains, part of the Tibetan Plateau. On the southeast, the pass known as the Saser La separates the Rimo Muztagh from the Saser Muztagh. The western border of the range is formed by the lower Siachen Glacier and its outflow, the Nubra River. Across this boundary lie the Saltoro Mountains and the Kailas Mountains.</obo:IAO_0000115>
        <oboInOwl:hasOBONamespace>GAZ</oboInOwl:hasOBONamespace>
        <oboInOwl:id>GAZ:00056917</oboInOwl:id>
        <rdfs:label>Rimo Muztagh</rdfs:label>
    </owl:NamedIndividual>
    


    <!-- http://purl.obolibrary.org/obo/GAZ_00056918 -->

    <owl:NamedIndividual rdf:about="http://purl.obolibrary.org/obo/GAZ_00056918">
        <obo:IAO_0000115>The easternmost subrange of the Karakoram range, in the Kashmir region of India. It is bounded on the south, east, and northeast by the Shyok River, which bends sharply around the southeast corner of the range. On the west it is separated from the neighboring Kailas Mountains by the Nubra River, while the pass known as the Saser La marks the boundary between this range and the Rimo Muztagh to the north. The Ladakh Range stands to the south of the Saser Muztagh, across the Shyok River. Notable glaciers of the Saser Muztagh include the North and South Shukpa Kunchang Glaciers, the Sakang Glacier, and the Chamshen Glacier.</obo:IAO_0000115>
        <oboInOwl:hasOBONamespace>GAZ</oboInOwl:hasOBONamespace>
        <oboInOwl:id>GAZ:00056918</oboInOwl:id>
        <rdfs:label>Saser Muztagh</rdfs:label>
    </owl:NamedIndividual>
    


    <!-- http://purl.obolibrary.org/obo/GAZ_00056919 -->

    <owl:NamedIndividual rdf:about="http://purl.obolibrary.org/obo/GAZ_00056919">
        <obo:RO_0001025 rdf:resource="http://purl.obolibrary.org/obo/GAZ_00018583"/>
        <obo:IAO_0000115>The largest Tehsil of the Northern Areas of Pakistan, it lies north of the Gilgit region and lies close to the Chinese border.</obo:IAO_0000115>
        <oboInOwl:hasOBONamespace>GAZ</oboInOwl:hasOBONamespace>
        <oboInOwl:id>GAZ:00056919</oboInOwl:id>
        <rdfs:label>Gojal Tehsil</rdfs:label>
    </owl:NamedIndividual>
    


    <!-- http://purl.obolibrary.org/obo/GAZ_00056948 -->

    <owl:NamedIndividual rdf:about="http://purl.obolibrary.org/obo/GAZ_00056948">
        <obo:RO_0001025 rdf:resource="http://purl.obolibrary.org/obo/GAZ_00005246"/>
        <obo:IAO_0000115>A desert located in western India and southeastern Pakistan. It lies mostly in the Indian State of Rajasthan, and extends into the southern portion of Haryana and Punjab states and into northern Gujarat state. In Pakistan, the desert covers eastern Sind province and the southeastern portion of Pakistan&apos;s Punjab province. In Pakistan&apos;s Punjab province it is known as the Cholistan Desert. Tharparker District of province Sindh Pakistan is also a part of Thar desert. The Thar Desert is bounded on the northwest by the Sutlej River, on the east by the Aravalli Range, on the south by the salt marsh known as the Rann of Kutch (parts of which are sometimes included in the Thar), and on the west by the Indus River. Its boundary to the large thorny steppe to the north is ill-defined. Rajasthan is divided into 33 districts and seven divisions.</obo:IAO_0000115>
        <oboInOwl:hasOBONamespace>GAZ</oboInOwl:hasOBONamespace>
        <oboInOwl:id>GAZ:00056948</oboInOwl:id>
        <rdfs:label>Thar Desert</rdfs:label>
    </owl:NamedIndividual>
    


    <!-- http://purl.obolibrary.org/obo/GAZ_00057344 -->

    <owl:NamedIndividual rdf:about="http://purl.obolibrary.org/obo/GAZ_00057344">
        <obo:IAO_0000115>A subrange of the Himalayas spanning part of the border between Tibet and Nepal. It contains four eight-thousanders: Mount Everest, Lhotse, Makalu, and Cho Oyu, as well as numerous other major peaks.</obo:IAO_0000115>
        <oboInOwl:hasOBONamespace>GAZ</oboInOwl:hasOBONamespace>
        <oboInOwl:id>GAZ:00057344</oboInOwl:id>
        <rdfs:label>Mahalangur Himal</rdfs:label>
    </owl:NamedIndividual>
    


    <!-- http://purl.obolibrary.org/obo/GAZ_00057359 -->

    <owl:NamedIndividual rdf:about="http://purl.obolibrary.org/obo/GAZ_00057359">
        <obo:IAO_0000115>A mountain range that is a southern branch of the main Himalayan chain of mountains. It rises spectacularly from the Indian plains to the north of Kangra and Mandi.</obo:IAO_0000115>
        <oboInOwl:hasOBONamespace>GAZ</oboInOwl:hasOBONamespace>
        <oboInOwl:id>GAZ:00057359</oboInOwl:id>
        <rdfs:label>Dhauladhar Range</rdfs:label>
    </owl:NamedIndividual>
    


    <!-- http://purl.obolibrary.org/obo/GAZ_00057373 -->

    <owl:NamedIndividual rdf:about="http://purl.obolibrary.org/obo/GAZ_00057373">
        <rdf:type rdf:resource="http://purl.obolibrary.org/obo/ENVO_00000106"/>
        <obo:IAO_0000115>A range of mountains that form a part of the Middle Himalayas across the two states of Jammu and Kashmir and Himachal Pradesh in India as well as Azad Kashmir, Pakistan.</obo:IAO_0000115>
        <oboInOwl:hasOBONamespace>GAZ</oboInOwl:hasOBONamespace>
        <oboInOwl:id>GAZ:00057373</oboInOwl:id>
        <rdfs:label>Pir Panjal Range</rdfs:label>
    </owl:NamedIndividual>
    


    <!-- http://purl.obolibrary.org/obo/GAZ_00057374 -->

    <owl:NamedIndividual rdf:about="http://purl.obolibrary.org/obo/GAZ_00057374">
        <obo:IAO_0000115>A mountain range that lies north of the Sub-Himalayan Range and south of the Great Himalayas. In Pakistan these mountains lie just north of Rawalpindi district covering the districts of Batagram, Mansehra and Abbottabad as well as Pakistan Administered Kashmir. These mountains are also home to Pakistan&apos;s important hill stations like Murree, Ghora Gali and Nathia Gali. It snows here during a few months of the year but there aren&apos;t any glaciers found in this region. The range continues east through the Indian states of Jammu and Kashmir, Himachal Pradesh, Uttarakhand, Uttar Pradesh. The range then enters the countries of Nepal and Bhutan, and then enters the eastern Indian states of West Bengal, Sikkim, Assam and Arunachal Pradesh.</obo:IAO_0000115>
        <oboInOwl:hasOBONamespace>GAZ</oboInOwl:hasOBONamespace>
        <oboInOwl:id>GAZ:00057374</oboInOwl:id>
        <rdfs:label>Lower Himalayan Range</rdfs:label>
    </owl:NamedIndividual>
    


    <!-- http://purl.obolibrary.org/obo/GAZ_00057375 -->

    <owl:NamedIndividual rdf:about="http://purl.obolibrary.org/obo/GAZ_00057375">
        <obo:IAO_0000115>The southernmost mountains in the Himalaya Range. Their average height varies between 600 to 1200 meters, and are not so high in altitude as compared to other mountain ranges in the Himalaya range. These mountains are well spread in Kashmir, in Pakistan however they are located south-east of the Rawalpindi district.</obo:IAO_0000115>
        <oboInOwl:hasOBONamespace>GAZ</oboInOwl:hasOBONamespace>
        <oboInOwl:id>GAZ:00057375</oboInOwl:id>
        <rdfs:label>Sub-Himalayan Range</rdfs:label>
    </owl:NamedIndividual>
    


    <!-- http://purl.obolibrary.org/obo/GAZ_00057376 -->

    <owl:NamedIndividual rdf:about="http://purl.obolibrary.org/obo/GAZ_00057376">
        <obo:IAO_0000115>A mountain range that lies north of the Lower Himalayan Range. These mountains are bounded by the Indus River in the north and the west as the river takes a southward turn at Sazin. The average height of the range is about 6000 meters. Some of the highest peaks in the world lie in these mountains e.g. Nanga Parbat (8126 meters), which is the sixth highest peak in the world and the second highest peak in Pakistan. Since the mountains are perpetually covered with snow there are many glaciers, with Rupal Glacier being the longest (17.6 km).</obo:IAO_0000115>
        <oboInOwl:hasOBONamespace>GAZ</oboInOwl:hasOBONamespace>
        <oboInOwl:id>GAZ:00057376</oboInOwl:id>
        <rdfs:label>Great Himalayas</rdfs:label>
    </owl:NamedIndividual>
    


    <!-- http://purl.obolibrary.org/obo/GAZ_00057421 -->

    <owl:NamedIndividual rdf:about="http://purl.obolibrary.org/obo/GAZ_00057421">
        <obo:IAO_0000115>A mountains in the north of Thailand that extend through Laos, Burma and China to link to the Himalayas, of which they may be considered foothills.</obo:IAO_0000115>
        <oboInOwl:hasOBONamespace>GAZ</oboInOwl:hasOBONamespace>
        <oboInOwl:id>GAZ:00057421</oboInOwl:id>
        <rdfs:label>Thai Highlands</rdfs:label>
    </owl:NamedIndividual>
    


    <!-- http://purl.obolibrary.org/obo/GAZ_00057450 -->

    <owl:NamedIndividual rdf:about="http://purl.obolibrary.org/obo/GAZ_00057450">
        <obo:RO_0001025 rdf:resource="http://purl.obolibrary.org/obo/GAZ_00004988"/>
        <obo:IAO_0000115>A mountain range in the Western Pamirs of Tajikistan. The length of the Akademiya Nauk Range is about 110 km. The crest of the range has an Alpine-like relief with 24 summits more than 6,000 m in height. The lowest saddle point, Kamaloyak is at the altitude of 4,340 m.</obo:IAO_0000115>
        <oboInOwl:hasOBONamespace>GAZ</oboInOwl:hasOBONamespace>
        <oboInOwl:id>GAZ:00057450</oboInOwl:id>
        <rdfs:label>Akademiya Nauk Range</rdfs:label>
    </owl:NamedIndividual>
    


    <!-- http://purl.obolibrary.org/obo/GAZ_00057453 -->

    <owl:NamedIndividual rdf:about="http://purl.obolibrary.org/obo/GAZ_00057453">
        <obo:IAO_0000115>A traditional designation for the portion of the Himalaya range between the eastern border of Bhutan, on the west, and the Great Bend of the Tsangpo River, on the east.</obo:IAO_0000115>
        <oboInOwl:hasOBONamespace>GAZ</oboInOwl:hasOBONamespace>
        <oboInOwl:id>GAZ:00057453</oboInOwl:id>
        <rdfs:label>Assam Himalaya</rdfs:label>
    </owl:NamedIndividual>
    


    <!-- http://purl.obolibrary.org/obo/GAZ_00057455 -->

    <owl:NamedIndividual rdf:about="http://purl.obolibrary.org/obo/GAZ_00057455">
        <obo:IAO_0000115>A sub-range of the Himalayan mountain range. It is located mostly in north-central Nepal, but some peaks lie on the border with Tibet. The Trisuli Gandaki valley on the east separates it from the Langtang Himal; the Budhi Gandaki valley and the Shyar Khola valley on the west separate it from the Sringi Himal and the Mansiri Himal (home of Manaslu, the nearest 8000m peak). The range lies about 70 km north-northwest of Kathmandu.</obo:IAO_0000115>
        <oboInOwl:hasOBONamespace>GAZ</oboInOwl:hasOBONamespace>
        <oboInOwl:id>GAZ:00057455</oboInOwl:id>
        <rdfs:label>Ganesh Himal</rdfs:label>
    </owl:NamedIndividual>
    


    <!-- http://purl.obolibrary.org/obo/GAZ_00057456 -->

    <owl:NamedIndividual rdf:about="http://purl.obolibrary.org/obo/GAZ_00057456">
        <oboInOwl:hasOBONamespace>GAZ</oboInOwl:hasOBONamespace>
        <oboInOwl:id>GAZ:00057456</oboInOwl:id>
        <rdfs:label>Langtang Himal</rdfs:label>
    </owl:NamedIndividual>
    


    <!-- http://purl.obolibrary.org/obo/GAZ_00057457 -->

    <owl:NamedIndividual rdf:about="http://purl.obolibrary.org/obo/GAZ_00057457">
        <oboInOwl:hasOBONamespace>GAZ</oboInOwl:hasOBONamespace>
        <oboInOwl:id>GAZ:00057457</oboInOwl:id>
        <rdfs:label>Sringi Himal</rdfs:label>
    </owl:NamedIndividual>
    


    <!-- http://purl.obolibrary.org/obo/GAZ_00057459 -->

    <owl:NamedIndividual rdf:about="http://purl.obolibrary.org/obo/GAZ_00057459">
        <obo:IAO_0000115>A small, high subrange of the Himalaya in north-central Nepal. It rises between the Marsyangdi River on the west, and the Burhi (Budhi) Gandaki on the east, and lies roughly 100 km northwest of Kathmandu. To the west lies the Annapurna Himal, and to the east is the Ganesh Himal.</obo:IAO_0000115>
        <oboInOwl:hasOBONamespace>GAZ</oboInOwl:hasOBONamespace>
        <oboInOwl:id>GAZ:00057459</oboInOwl:id>
        <rdfs:label>Mansiri Himal</rdfs:label>
    </owl:NamedIndividual>
    


    <!-- http://purl.obolibrary.org/obo/GAZ_00057460 -->

    <owl:NamedIndividual rdf:about="http://purl.obolibrary.org/obo/GAZ_00057460">
        <obo:IAO_0000115>A series of peaks in the Himalaya, a 55 km ong massif whose highest point, Annapurna I, stands at 8,091 m making it the 10th-highest summit in the world. It is located east of a great gorge cut through the Himalaya by the Kali Gandaki River, which separates it from the Dhaulagiri massif.</obo:IAO_0000115>
        <oboInOwl:hasOBONamespace>GAZ</oboInOwl:hasOBONamespace>
        <oboInOwl:id>GAZ:00057460</oboInOwl:id>
        <rdfs:label>Annapurna Himal</rdfs:label>
    </owl:NamedIndividual>
    


    <!-- http://purl.obolibrary.org/obo/GAZ_00057461 -->

    <owl:NamedIndividual rdf:about="http://purl.obolibrary.org/obo/GAZ_00057461">
        <obo:IAO_0000115>A small subrange of the Himalayan range in southern Tibet and the northwest corner of Nepal. It lies south of Lake Manasarowar. Its southern boundary is the Humla Karnali, a tributary of the Karnali, one of the major rivers of western Nepal. This river separates the range from the Gurans Himal to the south and the eastern Kumaon to the southwest. On the east, the pass known as Lapche La marks the dividing point between the Nalakankar Himal and the Chandi Himal. To the north and northwest, the range fades into the northern foothills of the Himalaya and the Tibetan Plateau.</obo:IAO_0000115>
        <oboInOwl:hasOBONamespace>GAZ</oboInOwl:hasOBONamespace>
        <oboInOwl:id>GAZ:00057461</oboInOwl:id>
        <rdfs:label>Nalakankar Himal</rdfs:label>
    </owl:NamedIndividual>
    


    <!-- http://purl.obolibrary.org/obo/GAZ_00057462 -->

    <owl:NamedIndividual rdf:about="http://purl.obolibrary.org/obo/GAZ_00057462">
        <obo:IAO_0000115>A sub-range of the Himalaya, located in north central Nepal and extending into south central Tibet. The range is bounded on the south by the Rolwaling Valley.</obo:IAO_0000115>
        <oboInOwl:hasOBONamespace>GAZ</oboInOwl:hasOBONamespace>
        <oboInOwl:id>GAZ:00057462</oboInOwl:id>
        <rdfs:label>Rolwaling Himal</rdfs:label>
    </owl:NamedIndividual>
    


    <!-- http://purl.obolibrary.org/obo/GAZ_00057463 -->

    <owl:NamedIndividual rdf:about="http://purl.obolibrary.org/obo/GAZ_00057463">
        <obo:IAO_0000115>A small subrange of the Himalaya in far western Nepal.</obo:IAO_0000115>
        <oboInOwl:hasOBONamespace>GAZ</oboInOwl:hasOBONamespace>
        <oboInOwl:id>GAZ:00057463</oboInOwl:id>
        <rdfs:label>Gurans Himal</rdfs:label>
    </owl:NamedIndividual>
    


    <!-- http://purl.obolibrary.org/obo/GAZ_00057464 -->

    <owl:NamedIndividual rdf:about="http://purl.obolibrary.org/obo/GAZ_00057464">
        <obo:IAO_0000115>A subrange of the Himalaya in the Dhawalagiri Zone of north central Nepal.</obo:IAO_0000115>
        <oboInOwl:hasOBONamespace>GAZ</oboInOwl:hasOBONamespace>
        <oboInOwl:id>GAZ:00057464</oboInOwl:id>
        <rdfs:label>Dhaulagiri Himal</rdfs:label>
    </owl:NamedIndividual>
    


    <!-- http://purl.obolibrary.org/obo/GAZ_00057491 -->

    <owl:NamedIndividual rdf:about="http://purl.obolibrary.org/obo/GAZ_00057491">
        <obo:RO_0001025 rdf:resource="http://purl.obolibrary.org/obo/GAZ_00004988"/>
        <obo:IAO_0000115>A mountain range of the Pamir Mountains (ancient Mount Imeon) between Kyrgyzstan and Tajikistan. Its northern end is the Alay Valley, and 150 miles to the south, it terminates into the valleys of Muksu and Markansu. The highest peak in the range is Lenin Peak.</obo:IAO_0000115>
        <oboInOwl:hasOBONamespace>GAZ</oboInOwl:hasOBONamespace>
        <oboInOwl:id>GAZ:00057491</oboInOwl:id>
        <rdfs:label>Trans-Alay Range</rdfs:label>
    </owl:NamedIndividual>
    


    <!-- http://purl.obolibrary.org/obo/GAZ_00057737 -->

    <owl:NamedIndividual rdf:about="http://purl.obolibrary.org/obo/GAZ_00057737">
        <obo:RO_0001025 rdf:resource="http://purl.obolibrary.org/obo/GAZ_00005249"/>
        <obo:IAO_0000115>A desert located in Punjab Province, Pakistan. It is a vast area mainly between the Jhelum and Sindh rivers near the Pothohar Plateau. Its total length from north to south is 190 miles, and its maximum breadth is 70 miles while minimum breadth is 20 miles. This region is divided into the districts of Bhakkar, Khushab, Mianwali, Jhang, Layyah, and Muzaffargarh. Its part in Jhang is on the left bank of the river Jehlum. Geographically, it resembles the deserts of Cholistan and Thar.</obo:IAO_0000115>
        <oboInOwl:hasOBONamespace>GAZ</oboInOwl:hasOBONamespace>
        <oboInOwl:id>GAZ:00057737</oboInOwl:id>
        <rdfs:label>Thal Desert</rdfs:label>
    </owl:NamedIndividual>
    


    <!-- http://purl.obolibrary.org/obo/GAZ_00057751 -->

    <owl:NamedIndividual rdf:about="http://purl.obolibrary.org/obo/GAZ_00057751">
        <obo:RO_0001025 rdf:resource="http://purl.obolibrary.org/obo/GAZ_00005249"/>
        <obo:IAO_0000115>A desert ecoregion of northern Pakistan. The Indus Valley desert covers an area of 19,500 km2 in northwestern Punjab Province, lying between the Chenab and Indus rivers.</obo:IAO_0000115>
        <oboInOwl:hasOBONamespace>GAZ</oboInOwl:hasOBONamespace>
        <oboInOwl:id>GAZ:00057751</oboInOwl:id>
        <rdfs:label>Indus Valley Desert</rdfs:label>
    </owl:NamedIndividual>
    


    <!-- http://purl.obolibrary.org/obo/GAZ_00058025 -->

    <owl:NamedIndividual rdf:about="http://purl.obolibrary.org/obo/GAZ_00058025">
        <obo:RO_0001025 rdf:resource="http://purl.obolibrary.org/obo/GAZ_00056902"/>
        <obo:IAO_0000115>A group of lakes high in the Hindu Kush Mountains of Central Afghanistan near the famous Buddhas of Bamyan. They were created by the carbon dioxide rich water oozing out of the faults and fractures to deposit calcium carbonate precipitate in the form of travertine walls that today store the water of these lakes. Band-e Amir is situated at approximately 75 km to the north-west of the ancient city of Bamyan, close the town of Yakawlang.</obo:IAO_0000115>
        <oboInOwl:hasOBONamespace>GAZ</oboInOwl:hasOBONamespace>
        <oboInOwl:id>GAZ:00058025</oboInOwl:id>
        <rdfs:label>Band-e Amir</rdfs:label>
    </owl:NamedIndividual>
    


    <!-- http://purl.obolibrary.org/obo/GAZ_00058026 -->

    <owl:NamedIndividual rdf:about="http://purl.obolibrary.org/obo/GAZ_00058026">
        <obo:RO_0001025 rdf:resource="http://purl.obolibrary.org/obo/GAZ_00058025"/>
        <obo:IAO_0000115>One of the Band-e Amir lakes.</obo:IAO_0000115>
        <oboInOwl:hasOBONamespace>GAZ</oboInOwl:hasOBONamespace>
        <oboInOwl:id>GAZ:00058026</oboInOwl:id>
        <rdfs:label>Band-e Haibat</rdfs:label>
    </owl:NamedIndividual>
    


    <!-- http://purl.obolibrary.org/obo/GAZ_00058027 -->

    <owl:NamedIndividual rdf:about="http://purl.obolibrary.org/obo/GAZ_00058027">
        <obo:RO_0001025 rdf:resource="http://purl.obolibrary.org/obo/GAZ_00058025"/>
        <obo:IAO_0000115>One of the Band-e Amir lakes.</obo:IAO_0000115>
        <oboInOwl:hasOBONamespace>GAZ</oboInOwl:hasOBONamespace>
        <oboInOwl:id>GAZ:00058027</oboInOwl:id>
        <rdfs:label>Band-e Qambar</rdfs:label>
    </owl:NamedIndividual>
    


    <!-- http://purl.obolibrary.org/obo/GAZ_00058028 -->

    <owl:NamedIndividual rdf:about="http://purl.obolibrary.org/obo/GAZ_00058028">
        <obo:RO_0001025 rdf:resource="http://purl.obolibrary.org/obo/GAZ_00058025"/>
        <obo:IAO_0000115>One of the Band-e Amir lakes.</obo:IAO_0000115>
        <oboInOwl:hasOBONamespace>GAZ</oboInOwl:hasOBONamespace>
        <oboInOwl:id>GAZ:00058028</oboInOwl:id>
        <rdfs:label>Band-e Zulfiqar</rdfs:label>
    </owl:NamedIndividual>
    


    <!-- http://purl.obolibrary.org/obo/GAZ_00058029 -->

    <owl:NamedIndividual rdf:about="http://purl.obolibrary.org/obo/GAZ_00058029">
        <obo:RO_0001025 rdf:resource="http://purl.obolibrary.org/obo/GAZ_00058025"/>
        <obo:IAO_0000115>One of the Band-e Amir lakes.</obo:IAO_0000115>
        <oboInOwl:hasOBONamespace>GAZ</oboInOwl:hasOBONamespace>
        <oboInOwl:id>GAZ:00058029</oboInOwl:id>
        <rdfs:label>Band-e Pudina</rdfs:label>
    </owl:NamedIndividual>
    


    <!-- http://purl.obolibrary.org/obo/GAZ_00058030 -->

    <owl:NamedIndividual rdf:about="http://purl.obolibrary.org/obo/GAZ_00058030">
        <obo:RO_0001025 rdf:resource="http://purl.obolibrary.org/obo/GAZ_00058025"/>
        <obo:IAO_0000115>One of the Band-e Amir lakes.</obo:IAO_0000115>
        <oboInOwl:hasOBONamespace>GAZ</oboInOwl:hasOBONamespace>
        <oboInOwl:id>GAZ:00058030</oboInOwl:id>
        <rdfs:label>Band-e Panir</rdfs:label>
    </owl:NamedIndividual>
    


    <!-- http://purl.obolibrary.org/obo/GAZ_00058031 -->

    <owl:NamedIndividual rdf:about="http://purl.obolibrary.org/obo/GAZ_00058031">
        <obo:RO_0001025 rdf:resource="http://purl.obolibrary.org/obo/GAZ_00058025"/>
        <obo:IAO_0000115>One of the Band-e Amir lakes.</obo:IAO_0000115>
        <oboInOwl:hasOBONamespace>GAZ</oboInOwl:hasOBONamespace>
        <oboInOwl:id>GAZ:00058031</oboInOwl:id>
        <rdfs:label>Band-e Gholaman</rdfs:label>
    </owl:NamedIndividual>
    


    <!-- http://purl.obolibrary.org/obo/GAZ_00058032 -->

    <owl:NamedIndividual rdf:about="http://purl.obolibrary.org/obo/GAZ_00058032">
        <obo:RO_0001025 rdf:resource="http://purl.obolibrary.org/obo/GAZ_00004988"/>
        <obo:IAO_0000115>A lake in the Pamir Mountains. It extends east to west for about 25 km. Along the western half of the lake runs the Afghan-Tajik border, turning south towards Concord Peak (5,469 m), about 15 km south of the lake. The lake&apos;s eastern half lies in Tajikistan. Out of the lake, towards the west, flows Pamir River.</obo:IAO_0000115>
        <oboInOwl:hasOBONamespace>GAZ</oboInOwl:hasOBONamespace>
        <oboInOwl:id>GAZ:00058032</oboInOwl:id>
        <rdfs:label>Zorkul</rdfs:label>
    </owl:NamedIndividual>
    


    <!-- http://purl.obolibrary.org/obo/GAZ_00058273 -->

    <owl:NamedIndividual rdf:about="http://purl.obolibrary.org/obo/GAZ_00058273">
        <obo:RO_0001025 rdf:resource="http://purl.obolibrary.org/obo/GAZ_00148807"/>
        <obo:IAO_0000115>A reservoir in the Bilaspur and Una Districts. It is 83 km from the town of Bilaspur, on the River Sutlej. Impounded by the Bhakra Dam.</obo:IAO_0000115>
        <oboInOwl:hasOBONamespace>GAZ</oboInOwl:hasOBONamespace>
        <oboInOwl:id>GAZ:00058273</oboInOwl:id>
        <rdfs:label>Gobind Sagar</rdfs:label>
    </owl:NamedIndividual>
    


    <!-- http://purl.obolibrary.org/obo/GAZ_00058274 -->

    <owl:NamedIndividual rdf:about="http://purl.obolibrary.org/obo/GAZ_00058274">
        <obo:IAO_0000115>A reservoir in Kangra District 170 km from Chandigarh. The sagar was made a reservoir in the 1970s by the construction of a dam in a wetland zone in the Siwalik Hills at an altitude of 350 to 500 m. A Ramsar Site.</obo:IAO_0000115>
        <oboInOwl:hasOBONamespace>GAZ</oboInOwl:hasOBONamespace>
        <oboInOwl:id>GAZ:00058274</oboInOwl:id>
        <rdfs:label>Maharana Pratap Sagar</rdfs:label>
    </owl:NamedIndividual>
    


    <!-- http://purl.obolibrary.org/obo/GAZ_00058281 -->

    <owl:NamedIndividual rdf:about="http://purl.obolibrary.org/obo/GAZ_00058281">
        <obo:IAO_0000115>A reservoir situated in Mandi district. The lake diverts the water from River Beas into the River Satluj.</obo:IAO_0000115>
        <oboInOwl:hasOBONamespace>GAZ</oboInOwl:hasOBONamespace>
        <oboInOwl:id>GAZ:00058281</oboInOwl:id>
        <rdfs:label>Pandoh Lake</rdfs:label>
    </owl:NamedIndividual>
    


    <!-- http://purl.obolibrary.org/obo/GAZ_00058285 -->

    <owl:NamedIndividual rdf:about="http://purl.obolibrary.org/obo/GAZ_00058285">
        <obo:IAO_0000115>A freshwater lake located between the cities of Sopore and Bandipore. The lake was formed as a result of tectonic activity and is the largest freshwater lake in India. The River Jhelum feeds into the lake, which acts as a natural flood reservoir.</obo:IAO_0000115>
        <oboInOwl:hasOBONamespace>GAZ</oboInOwl:hasOBONamespace>
        <oboInOwl:id>GAZ:00058285</oboInOwl:id>
        <rdfs:label>Wular Lake</rdfs:label>
    </owl:NamedIndividual>
    


    <!-- http://purl.obolibrary.org/obo/GAZ_00058368 -->

    <owl:NamedIndividual rdf:about="http://purl.obolibrary.org/obo/GAZ_00058368">
        <obo:IAO_0000115>The southernmost and geologically youngest east-west mountain chain of the Himalayan System. The Sivalik Hills crest at 900 to 1,200 meters and have many sub-ranges. They extend 1,600 km from the Teesta River in Sikkim, westward through Nepal and Uttarakhand, continuing into Kashmir and Northern Pakistan. The Mohan Pass is the principal pass accessing the Sivalik Hills from Saharanpur in Uttar Pradesh to Dehra and the hill station of Mussoorie in Uttarakhand. Eastward they are cut through at wide intervals by large rivers flowing south from the Himalaya.</obo:IAO_0000115>
        <oboInOwl:hasOBONamespace>GAZ</oboInOwl:hasOBONamespace>
        <oboInOwl:id>GAZ:00058368</oboInOwl:id>
        <rdfs:label>Sivalik Hills</rdfs:label>
    </owl:NamedIndividual>
    


    <!-- http://purl.obolibrary.org/obo/GAZ_00058373 -->

    <owl:NamedIndividual rdf:about="http://purl.obolibrary.org/obo/GAZ_00058373">
        <obo:RO_0001025 rdf:resource="http://purl.obolibrary.org/obo/GAZ_00057460"/>
        <obo:IAO_0000115>One of the highest lakes in the world in the Annapurna Himal. A tarn, a lake caused by glacial activity.</obo:IAO_0000115>
        <oboInOwl:hasOBONamespace>GAZ</oboInOwl:hasOBONamespace>
        <oboInOwl:id>GAZ:00058373</oboInOwl:id>
        <rdfs:label>Tilicho Lake</rdfs:label>
    </owl:NamedIndividual>
    


    <!-- http://purl.obolibrary.org/obo/GAZ_00058422 -->

    <owl:NamedIndividual rdf:about="http://purl.obolibrary.org/obo/GAZ_00058422">
        <obo:RO_0001025 rdf:resource="http://purl.obolibrary.org/obo/GAZ_00058423"/>
        <obo:IAO_0000115>A high-altitude lake (elevation 5,027 m) in the Kaghan Valley in the Mansehra District of the North-West Frontier Province of Pakistan. It is near Malika Parbat in the Himalayan range.</obo:IAO_0000115>
        <oboInOwl:hasOBONamespace>GAZ</oboInOwl:hasOBONamespace>
        <oboInOwl:id>GAZ:00058422</oboInOwl:id>
        <rdfs:label>Ansoo Lake</rdfs:label>
    </owl:NamedIndividual>
    


    <!-- http://purl.obolibrary.org/obo/GAZ_00058423 -->

    <owl:NamedIndividual rdf:about="http://purl.obolibrary.org/obo/GAZ_00058423">
        <obo:RO_0001025 rdf:resource="http://purl.obolibrary.org/obo/GAZ_00400027"/>
        <obo:IAO_0000115>A valley in the Mansehra District of the North-West Frontier Province of Pakistan.</obo:IAO_0000115>
        <oboInOwl:hasOBONamespace>GAZ</oboInOwl:hasOBONamespace>
        <oboInOwl:id>GAZ:00058423</oboInOwl:id>
        <rdfs:label>Kaghan Valley</rdfs:label>
    </owl:NamedIndividual>
    


    <!-- http://purl.obolibrary.org/obo/GAZ_00058424 -->

    <owl:NamedIndividual rdf:about="http://purl.obolibrary.org/obo/GAZ_00058424">
        <obo:RO_0001025 rdf:resource="http://purl.obolibrary.org/obo/GAZ_00058425"/>
        <obo:IAO_0000115>A saline lake in the Northern Areas of Pakistan. It lies approximately 2 km to the north of Ghulkin.</obo:IAO_0000115>
        <oboInOwl:hasOBONamespace>GAZ</oboInOwl:hasOBONamespace>
        <oboInOwl:id>GAZ:00058424</oboInOwl:id>
        <rdfs:label>Borith Lake</rdfs:label>
    </owl:NamedIndividual>
    


    <!-- http://purl.obolibrary.org/obo/GAZ_00058425 -->

    <owl:NamedIndividual rdf:about="http://purl.obolibrary.org/obo/GAZ_00058425">
        <obo:RO_0001025 rdf:resource="http://purl.obolibrary.org/obo/GAZ_00018575"/>
        <obo:IAO_0000115>A mountainous valley near Gilgit in the Northern Areas of Pakistan.</obo:IAO_0000115>
        <oboInOwl:hasOBONamespace>GAZ</oboInOwl:hasOBONamespace>
        <oboInOwl:id>GAZ:00058425</oboInOwl:id>
        <rdfs:label>Hunza Valley</rdfs:label>
    </owl:NamedIndividual>
    


    <!-- http://purl.obolibrary.org/obo/GAZ_00058426 -->

    <owl:NamedIndividual rdf:about="http://purl.obolibrary.org/obo/GAZ_00058426">
        <obo:RO_0001025 rdf:resource="http://purl.obolibrary.org/obo/GAZ_00058423"/>
        <obo:IAO_0000115>A lake that lies in the extreme north of Kaghan Valley.</obo:IAO_0000115>
        <oboInOwl:hasOBONamespace>GAZ</oboInOwl:hasOBONamespace>
        <oboInOwl:id>GAZ:00058426</oboInOwl:id>
        <rdfs:label>Dudipatsar Lake</rdfs:label>
    </owl:NamedIndividual>
    


    <!-- http://purl.obolibrary.org/obo/GAZ_00058427 -->

    <owl:NamedIndividual rdf:about="http://purl.obolibrary.org/obo/GAZ_00058427">
        <obo:RO_0001025 rdf:resource="http://purl.obolibrary.org/obo/GAZ_00058423"/>
        <obo:IAO_0000115>The main contributory to the Kunhar River that runs through Kaghan valley.</obo:IAO_0000115>
        <oboInOwl:hasOBONamespace>GAZ</oboInOwl:hasOBONamespace>
        <oboInOwl:id>GAZ:00058427</oboInOwl:id>
        <rdfs:label>Lake Lulusar</rdfs:label>
    </owl:NamedIndividual>
    


    <!-- http://purl.obolibrary.org/obo/GAZ_00058428 -->

    <owl:NamedIndividual rdf:about="http://purl.obolibrary.org/obo/GAZ_00058428">
        <obo:RO_0001025 rdf:resource="http://purl.obolibrary.org/obo/GAZ_00253152"/>
        <obo:IAO_0000115>A freshwater lake located in Thatta District, Sindh, Pakistan. The lake was originally a saline lagoon formed by seasonal rainwater collecting in a shallow depression. However, in the late 1930s, the lagoon was converted into a water storage reservoir by diverting the Jam Branch Canal into it.</obo:IAO_0000115>
        <oboInOwl:hasOBONamespace>GAZ</oboInOwl:hasOBONamespace>
        <oboInOwl:id>GAZ:00058428</oboInOwl:id>
        <rdfs:label>Haleji Lake</rdfs:label>
    </owl:NamedIndividual>
    


    <!-- http://purl.obolibrary.org/obo/GAZ_00058429 -->

    <owl:NamedIndividual rdf:about="http://purl.obolibrary.org/obo/GAZ_00058429">
        <obo:RO_0001025 rdf:resource="http://purl.obolibrary.org/obo/GAZ_00400006"/>
        <obo:IAO_0000115>A lake 10 km east of Quetta city in Pakistan.</obo:IAO_0000115>
        <oboInOwl:hasOBONamespace>GAZ</oboInOwl:hasOBONamespace>
        <oboInOwl:id>GAZ:00058429</oboInOwl:id>
        <rdfs:label>Hanna Lake</rdfs:label>
    </owl:NamedIndividual>
    


    <!-- http://purl.obolibrary.org/obo/GAZ_00058430 -->

    <owl:NamedIndividual rdf:about="http://purl.obolibrary.org/obo/GAZ_00058430">
        <obo:RO_0001025 rdf:resource="http://purl.obolibrary.org/obo/GAZ_00058423"/>
        <obo:IAO_0000115>A lake in the Kaghan Valley.</obo:IAO_0000115>
        <oboInOwl:hasOBONamespace>GAZ</oboInOwl:hasOBONamespace>
        <oboInOwl:id>GAZ:00058430</oboInOwl:id>
        <rdfs:label>Dudibach Lake</rdfs:label>
    </owl:NamedIndividual>
    


    <!-- http://purl.obolibrary.org/obo/GAZ_00058431 -->

    <owl:NamedIndividual rdf:about="http://purl.obolibrary.org/obo/GAZ_00058431">
        <obo:RO_0001025 rdf:resource="http://purl.obolibrary.org/obo/GAZ_00018575"/>
        <obo:IAO_0000115>A high mountain valley in the Himalaya mountains, in the northwest region of Gilgit in the Northern Areas of Pakistan. Ishkoman is connected to the Yasin Valley by a high mountain pass.</obo:IAO_0000115>
        <oboInOwl:hasOBONamespace>GAZ</oboInOwl:hasOBONamespace>
        <oboInOwl:id>GAZ:00058431</oboInOwl:id>
        <rdfs:label>Ishkoman Valley</rdfs:label>
    </owl:NamedIndividual>
    


    <!-- http://purl.obolibrary.org/obo/GAZ_00058432 -->

    <owl:NamedIndividual rdf:about="http://purl.obolibrary.org/obo/GAZ_00058432">
        <obo:RO_0001025 rdf:resource="http://purl.obolibrary.org/obo/GAZ_00018575"/>
        <obo:IAO_0000115>A high mountain valley in the Hindu Kush mountains, in the northwest region of Gilgit in the Northern Areas of Pakistan. Yasin is separated from the Ishkoman Valley by a high mountain pass.</obo:IAO_0000115>
        <oboInOwl:hasOBONamespace>GAZ</oboInOwl:hasOBONamespace>
        <oboInOwl:id>GAZ:00058432</oboInOwl:id>
        <rdfs:label>Yasin Valley</rdfs:label>
    </owl:NamedIndividual>
    


    <!-- http://purl.obolibrary.org/obo/GAZ_00058433 -->

    <owl:NamedIndividual rdf:about="http://purl.obolibrary.org/obo/GAZ_00058433">
        <obo:RO_0001025 rdf:resource="http://purl.obolibrary.org/obo/GAZ_00058431"/>
        <obo:RO_0001025 rdf:resource="http://purl.obolibrary.org/obo/GAZ_00058432"/>
        <obo:IAO_0000115>A lake in the Yasin and Ishkoman Valleys.</obo:IAO_0000115>
        <oboInOwl:hasOBONamespace>GAZ</oboInOwl:hasOBONamespace>
        <oboInOwl:id>GAZ:00058433</oboInOwl:id>
        <rdfs:label>Attar Lake</rdfs:label>
    </owl:NamedIndividual>
    


    <!-- http://purl.obolibrary.org/obo/GAZ_00058434 -->

    <owl:NamedIndividual rdf:about="http://purl.obolibrary.org/obo/GAZ_00058434">
        <rdf:type rdf:resource="http://purl.obolibrary.org/obo/ENVO_00000856"/>
        <obo:RO_0001025 rdf:resource="http://purl.obolibrary.org/obo/GAZ_00018583"/>
        <obo:IAO_0000115>A populated place. A town 45 km from Giglit.</obo:IAO_0000115>
        <oboInOwl:hasOBONamespace>GAZ</oboInOwl:hasOBONamespace>
        <oboInOwl:id>GAZ:00058434</oboInOwl:id>
        <rdfs:label>Juglot Gilgit</rdfs:label>
    </owl:NamedIndividual>
    


    <!-- http://purl.obolibrary.org/obo/GAZ_00058435 -->

    <owl:NamedIndividual rdf:about="http://purl.obolibrary.org/obo/GAZ_00058435">
        <obo:RO_0001025 rdf:resource="http://purl.obolibrary.org/obo/GAZ_00058434"/>
        <obo:IAO_0000115>A lake.</obo:IAO_0000115>
        <oboInOwl:hasOBONamespace>GAZ</oboInOwl:hasOBONamespace>
        <oboInOwl:id>GAZ:00058435</oboInOwl:id>
        <rdfs:label>Gasho Pahott Lake</rdfs:label>
    </owl:NamedIndividual>
    


    <!-- http://purl.obolibrary.org/obo/GAZ_00058436 -->

    <owl:NamedIndividual rdf:about="http://purl.obolibrary.org/obo/GAZ_00058436">
        <obo:RO_0001025 rdf:resource="http://purl.obolibrary.org/obo/GAZ_00058437"/>
        <obo:IAO_0000115>One of the Kachura Lakes.</obo:IAO_0000115>
        <oboInOwl:hasOBONamespace>GAZ</oboInOwl:hasOBONamespace>
        <oboInOwl:id>GAZ:00058436</oboInOwl:id>
        <rdfs:label>Lower Kachura Lake</rdfs:label>
    </owl:NamedIndividual>
    


    <!-- http://purl.obolibrary.org/obo/GAZ_00058437 -->

    <owl:NamedIndividual rdf:about="http://purl.obolibrary.org/obo/GAZ_00058437">
        <obo:RO_0001025 rdf:resource="http://purl.obolibrary.org/obo/GAZ_00018580"/>
        <obo:IAO_0000115>Two of the lakes in Skardu District.</obo:IAO_0000115>
        <oboInOwl:hasOBONamespace>GAZ</oboInOwl:hasOBONamespace>
        <oboInOwl:id>GAZ:00058437</oboInOwl:id>
        <rdfs:label>Kachura Lakes</rdfs:label>
    </owl:NamedIndividual>
    


    <!-- http://purl.obolibrary.org/obo/GAZ_00058438 -->

    <owl:NamedIndividual rdf:about="http://purl.obolibrary.org/obo/GAZ_00058438">
        <obo:RO_0001025 rdf:resource="http://purl.obolibrary.org/obo/GAZ_00058437"/>
        <obo:IAO_0000115>One of the Kachura Lakes.</obo:IAO_0000115>
        <oboInOwl:hasOBONamespace>GAZ</oboInOwl:hasOBONamespace>
        <oboInOwl:id>GAZ:00058438</oboInOwl:id>
        <rdfs:label>Upper Kachura Lake</rdfs:label>
    </owl:NamedIndividual>
    


    <!-- http://purl.obolibrary.org/obo/GAZ_00058439 -->

    <owl:NamedIndividual rdf:about="http://purl.obolibrary.org/obo/GAZ_00058439">
        <obo:RO_0001025 rdf:resource="http://purl.obolibrary.org/obo/GAZ_00400081"/>
        <obo:IAO_0000115>A saline lake.</obo:IAO_0000115>
        <oboInOwl:hasOBONamespace>GAZ</oboInOwl:hasOBONamespace>
        <oboInOwl:id>GAZ:00058439</oboInOwl:id>
        <rdfs:label>Kallar Kahar Lake</rdfs:label>
    </owl:NamedIndividual>
    


    <!-- http://purl.obolibrary.org/obo/GAZ_00058440 -->

    <owl:NamedIndividual rdf:about="http://purl.obolibrary.org/obo/GAZ_00058440">
        <obo:RO_0001025 rdf:resource="http://purl.obolibrary.org/obo/GAZ_00018576"/>
        <obo:IAO_0000115>A lake.</obo:IAO_0000115>
        <oboInOwl:hasOBONamespace>GAZ</oboInOwl:hasOBONamespace>
        <oboInOwl:id>GAZ:00058440</oboInOwl:id>
        <rdfs:label>Karambar Lake</rdfs:label>
    </owl:NamedIndividual>
    


    <!-- http://purl.obolibrary.org/obo/GAZ_00058441 -->

    <owl:NamedIndividual rdf:about="http://purl.obolibrary.org/obo/GAZ_00058441">
        <obo:RO_0001025 rdf:resource="http://purl.obolibrary.org/obo/GAZ_00018576"/>
        <obo:IAO_0000115>A lake.</obo:IAO_0000115>
        <oboInOwl:hasOBONamespace>GAZ</oboInOwl:hasOBONamespace>
        <oboInOwl:id>GAZ:00058441</oboInOwl:id>
        <rdfs:label>Khalti Lake</rdfs:label>
    </owl:NamedIndividual>
    


    <!-- http://purl.obolibrary.org/obo/GAZ_00058442 -->

    <owl:NamedIndividual rdf:about="http://purl.obolibrary.org/obo/GAZ_00058442">
        <obo:RO_0001025 rdf:resource="http://purl.obolibrary.org/obo/GAZ_00253163"/>
        <obo:IAO_0000115>A man-made freshwater lake located in Thatta, Sindh, Pakistan. It was created in the 1930s from two smaller lakes, Kinjhar and Kairi, by the construction of a dam at Chilia Bangla and a 12 km long embankment (bund) along the east side.</obo:IAO_0000115>
        <oboInOwl:hasOBONamespace>GAZ</oboInOwl:hasOBONamespace>
        <oboInOwl:id>GAZ:00058442</oboInOwl:id>
        <rdfs:label>Kalri Lake</rdfs:label>
    </owl:NamedIndividual>
    


    <!-- http://purl.obolibrary.org/obo/GAZ_00058443 -->

    <owl:NamedIndividual rdf:about="http://purl.obolibrary.org/obo/GAZ_00058443">
        <obo:RO_0001025 rdf:resource="http://purl.obolibrary.org/obo/GAZ_00005256"/>
        <obo:IAO_0000115>A valley in the North-West Frontier Province.</obo:IAO_0000115>
        <oboInOwl:hasOBONamespace>GAZ</oboInOwl:hasOBONamespace>
        <oboInOwl:id>GAZ:00058443</oboInOwl:id>
        <rdfs:label>Swat Valley</rdfs:label>
    </owl:NamedIndividual>
    


    <!-- http://purl.obolibrary.org/obo/GAZ_00058444 -->

    <owl:NamedIndividual rdf:about="http://purl.obolibrary.org/obo/GAZ_00058444">
        <obo:RO_0001025 rdf:resource="http://purl.obolibrary.org/obo/GAZ_00058443"/>
        <obo:IAO_0000115>A lake.</obo:IAO_0000115>
        <oboInOwl:hasOBONamespace>GAZ</oboInOwl:hasOBONamespace>
        <oboInOwl:id>GAZ:00058444</oboInOwl:id>
        <rdfs:label>Kundol Lake</rdfs:label>
    </owl:NamedIndividual>
    


    <!-- http://purl.obolibrary.org/obo/GAZ_00058445 -->

    <owl:NamedIndividual rdf:about="http://purl.obolibrary.org/obo/GAZ_00058445">
        <obo:RO_0001025 rdf:resource="http://purl.obolibrary.org/obo/GAZ_00005256"/>
        <oboInOwl:hasOBONamespace>GAZ</oboInOwl:hasOBONamespace>
        <oboInOwl:id>GAZ:00058445</oboInOwl:id>
        <rdfs:label>Haramosh Valley</rdfs:label>
    </owl:NamedIndividual>
    


    <!-- http://purl.obolibrary.org/obo/GAZ_00058446 -->

    <owl:NamedIndividual rdf:about="http://purl.obolibrary.org/obo/GAZ_00058446">
        <obo:RO_0001025 rdf:resource="http://purl.obolibrary.org/obo/GAZ_00058445"/>
        <obo:IAO_0000115>A lake.</obo:IAO_0000115>
        <oboInOwl:hasOBONamespace>GAZ</oboInOwl:hasOBONamespace>
        <oboInOwl:id>GAZ:00058446</oboInOwl:id>
        <rdfs:label>Kutwal Lake</rdfs:label>
    </owl:NamedIndividual>
    


    <!-- http://purl.obolibrary.org/obo/GAZ_00058447 -->

    <owl:NamedIndividual rdf:about="http://purl.obolibrary.org/obo/GAZ_00058447">
        <obo:RO_0001025 rdf:resource="http://purl.obolibrary.org/obo/GAZ_00400021"/>
        <obo:IAO_0000115>A lake.</obo:IAO_0000115>
        <oboInOwl:hasOBONamespace>GAZ</oboInOwl:hasOBONamespace>
        <oboInOwl:id>GAZ:00058447</oboInOwl:id>
        <rdfs:label>Marav Lake</rdfs:label>
    </owl:NamedIndividual>
    


    <!-- http://purl.obolibrary.org/obo/GAZ_00058448 -->

    <owl:NamedIndividual rdf:about="http://purl.obolibrary.org/obo/GAZ_00058448">
        <rdf:type rdf:resource="http://purl.obolibrary.org/obo/ENVO_00000856"/>
        <obo:RO_0001025 rdf:resource="http://purl.obolibrary.org/obo/GAZ_00080341"/>
    </owl:NamedIndividual>
    


    <!-- http://purl.obolibrary.org/obo/GAZ_00058449 -->

    <owl:NamedIndividual rdf:about="http://purl.obolibrary.org/obo/GAZ_00058449">
        <obo:RO_0001025 rdf:resource="http://purl.obolibrary.org/obo/GAZ_00058448"/>
        <obo:IAO_0000115>An artificial reservoir located west of the Indus River in Sindh. The lake was created in the 1930&apos;s when the Sukkur Barrage was constructed on the river Indus. The lake is fed by two canals, the Aral Wah Canal and the Danister Canal from the river Indus. The lake collects water from numerous small streams in the Kirthar Mountains and empties into the Indus River.</obo:IAO_0000115>
        <oboInOwl:hasOBONamespace>GAZ</oboInOwl:hasOBONamespace>
        <oboInOwl:id>GAZ:00058449</oboInOwl:id>
        <rdfs:label>Lake Manchar</rdfs:label>
    </owl:NamedIndividual>
    


    <!-- http://purl.obolibrary.org/obo/GAZ_00058450 -->

    <owl:NamedIndividual rdf:about="http://purl.obolibrary.org/obo/GAZ_00058450">
        <obo:RO_0001025 rdf:resource="http://purl.obolibrary.org/obo/GAZ_00018583"/>
        <obo:IAO_0000115>A valley near Gilgit and Hunza in the Northern Areas of Pakistan. Naltar is 40 km from Gilgit.</obo:IAO_0000115>
        <oboInOwl:hasOBONamespace>GAZ</oboInOwl:hasOBONamespace>
        <oboInOwl:id>GAZ:00058450</oboInOwl:id>
        <rdfs:label>Naltar Valley</rdfs:label>
    </owl:NamedIndividual>
    


    <!-- http://purl.obolibrary.org/obo/GAZ_00058451 -->

    <owl:NamedIndividual rdf:about="http://purl.obolibrary.org/obo/GAZ_00058451">
        <obo:RO_0001025 rdf:resource="http://purl.obolibrary.org/obo/GAZ_00058450"/>
        <obo:IAO_0000115>A lake.</obo:IAO_0000115>
        <oboInOwl:hasOBONamespace>GAZ</oboInOwl:hasOBONamespace>
        <oboInOwl:id>GAZ:00058451</oboInOwl:id>
        <rdfs:label>Naltar Lake</rdfs:label>
    </owl:NamedIndividual>
    


    <!-- http://purl.obolibrary.org/obo/GAZ_00058452 -->

    <owl:NamedIndividual rdf:about="http://purl.obolibrary.org/obo/GAZ_00058452">
        <obo:RO_0001025 rdf:resource="http://purl.obolibrary.org/obo/GAZ_00400056"/>
        <obo:IAO_0000115>A reservoir lake located in the Namal valley in Mianwali, Punjab, Pakistan. This lake was created when Namal Dam was constructed in 1913.</obo:IAO_0000115>
        <oboInOwl:hasOBONamespace>GAZ</oboInOwl:hasOBONamespace>
        <oboInOwl:id>GAZ:00058452</oboInOwl:id>
        <rdfs:label>Namal Lake</rdfs:label>
    </owl:NamedIndividual>
    


    <!-- http://purl.obolibrary.org/obo/GAZ_00058453 -->

    <owl:NamedIndividual rdf:about="http://purl.obolibrary.org/obo/GAZ_00058453">
        <obo:RO_0001025 rdf:resource="http://purl.obolibrary.org/obo/GAZ_00018576"/>
        <oboInOwl:hasOBONamespace>GAZ</oboInOwl:hasOBONamespace>
        <oboInOwl:id>GAZ:00058453</oboInOwl:id>
        <rdfs:label>Fander Valley</rdfs:label>
    </owl:NamedIndividual>
    


    <!-- http://purl.obolibrary.org/obo/GAZ_00058454 -->

    <owl:NamedIndividual rdf:about="http://purl.obolibrary.org/obo/GAZ_00058454">
        <obo:RO_0001025 rdf:resource="http://purl.obolibrary.org/obo/GAZ_00058453"/>
        <obo:IAO_0000115>A lake.</obo:IAO_0000115>
        <oboInOwl:hasOBONamespace>GAZ</oboInOwl:hasOBONamespace>
        <oboInOwl:id>GAZ:00058454</oboInOwl:id>
        <rdfs:label>Phandar Lake</rdfs:label>
    </owl:NamedIndividual>
    


    <!-- http://purl.obolibrary.org/obo/GAZ_00058455 -->

    <owl:NamedIndividual rdf:about="http://purl.obolibrary.org/obo/GAZ_00058455">
        <obo:RO_0001025 rdf:resource="http://purl.obolibrary.org/obo/GAZ_00018578"/>
        <obo:IAO_0000115>A lake near Astore in Northern Areas, Pakistan.</obo:IAO_0000115>
        <oboInOwl:hasOBONamespace>GAZ</oboInOwl:hasOBONamespace>
        <oboInOwl:id>GAZ:00058455</oboInOwl:id>
        <rdfs:label>Rama Lake</rdfs:label>
    </owl:NamedIndividual>
    


    <!-- http://purl.obolibrary.org/obo/GAZ_00058456 -->

    <owl:NamedIndividual rdf:about="http://purl.obolibrary.org/obo/GAZ_00058456">
        <obo:RO_0001025 rdf:resource="http://purl.obolibrary.org/obo/GAZ_00012614"/>
        <obo:IAO_0000115>A national park located in Northern Pakistan at the foothills of the Himalayas.</obo:IAO_0000115>
        <oboInOwl:hasOBONamespace>GAZ</oboInOwl:hasOBONamespace>
        <oboInOwl:id>GAZ:00058456</oboInOwl:id>
        <rdfs:label>Margalla Hills National Park</rdfs:label>
    </owl:NamedIndividual>
    


    <!-- http://purl.obolibrary.org/obo/GAZ_00058457 -->

    <owl:NamedIndividual rdf:about="http://purl.obolibrary.org/obo/GAZ_00058457">
        <obo:RO_0001025 rdf:resource="http://purl.obolibrary.org/obo/GAZ_00253182"/>
        <obo:IAO_0000115>An artificial reservoir in Pakistan that provides the water needs for the cities of Rawalpindi and Islamabad. This artificial lake covers an area of 8.8 km2. Rawal Lake is located within an isolated section of the Margalla Hills National Park.</obo:IAO_0000115>
        <oboInOwl:hasOBONamespace>GAZ</oboInOwl:hasOBONamespace>
        <oboInOwl:id>GAZ:00058457</oboInOwl:id>
        <rdfs:label>Rawal Lake</rdfs:label>
    </owl:NamedIndividual>
    


    <!-- http://purl.obolibrary.org/obo/GAZ_00058458 -->

    <owl:NamedIndividual rdf:about="http://purl.obolibrary.org/obo/GAZ_00058458">
        <obo:RO_0001025 rdf:resource="http://purl.obolibrary.org/obo/GAZ_00018583"/>
        <obo:IAO_0000115>A high altitude glacial lake located near Rush Pari Peak (5,098 m).</obo:IAO_0000115>
        <oboInOwl:hasOBONamespace>GAZ</oboInOwl:hasOBONamespace>
        <oboInOwl:id>GAZ:00058458</oboInOwl:id>
        <rdfs:label>Rush Lake</rdfs:label>
    </owl:NamedIndividual>
    


    <!-- http://purl.obolibrary.org/obo/GAZ_00058459 -->

    <owl:NamedIndividual rdf:about="http://purl.obolibrary.org/obo/GAZ_00058459">
        <obo:RO_0001025 rdf:resource="http://purl.obolibrary.org/obo/GAZ_00058423"/>
        <obo:IAO_0000115>A lake located at the northern end of the Kaghan Valley near Naran.</obo:IAO_0000115>
        <oboInOwl:hasOBONamespace>GAZ</oboInOwl:hasOBONamespace>
        <oboInOwl:id>GAZ:00058459</oboInOwl:id>
        <rdfs:label>Lake Saiful Muluk</rdfs:label>
    </owl:NamedIndividual>
    


    <!-- http://purl.obolibrary.org/obo/GAZ_00058460 -->

    <owl:NamedIndividual rdf:about="http://purl.obolibrary.org/obo/GAZ_00058460">
        <obo:RO_0001025 rdf:resource="http://purl.obolibrary.org/obo/GAZ_00058423"/>
        <obo:IAO_0000115>A lake.</obo:IAO_0000115>
        <oboInOwl:hasOBONamespace>GAZ</oboInOwl:hasOBONamespace>
        <oboInOwl:id>GAZ:00058460</oboInOwl:id>
        <rdfs:label>Saral Lake</rdfs:label>
    </owl:NamedIndividual>
    


    <!-- http://purl.obolibrary.org/obo/GAZ_00058461 -->

    <owl:NamedIndividual rdf:about="http://purl.obolibrary.org/obo/GAZ_00058461">
        <obo:RO_0001025 rdf:resource="http://purl.obolibrary.org/obo/GAZ_00018580"/>
        <obo:IAO_0000115>A lake in Skardu Valley.</obo:IAO_0000115>
        <oboInOwl:hasOBONamespace>GAZ</oboInOwl:hasOBONamespace>
        <oboInOwl:id>GAZ:00058461</oboInOwl:id>
        <rdfs:label>Satpara Lake</rdfs:label>
    </owl:NamedIndividual>
    


    <!-- http://purl.obolibrary.org/obo/GAZ_00058462 -->

    <owl:NamedIndividual rdf:about="http://purl.obolibrary.org/obo/GAZ_00058462">
        <obo:RO_0001025 rdf:resource="http://purl.obolibrary.org/obo/GAZ_00018580"/>
        <obo:IAO_0000115>A high-altitude glacial basin in the Karakoram mountain range in the Northern Areas of Pakistan. Snow Lake is located 4,877 m above sea level, and is approximately 16 km wide. The basin lies at the head of the Biafo and Hispar glaciers.</obo:IAO_0000115>
        <oboInOwl:hasOBONamespace>GAZ</oboInOwl:hasOBONamespace>
        <oboInOwl:id>GAZ:00058462</oboInOwl:id>
        <rdfs:label>Snow Lake</rdfs:label>
    </owl:NamedIndividual>
    


    <!-- http://purl.obolibrary.org/obo/GAZ_00058463 -->

    <owl:NamedIndividual rdf:about="http://purl.obolibrary.org/obo/GAZ_00058463">
        <obo:RO_0001025 rdf:resource="http://purl.obolibrary.org/obo/GAZ_00018580"/>
        <obo:IAO_0000115>A national park located above the tree line and at an average height of 13,500 feet above sea level.</obo:IAO_0000115>
        <oboInOwl:hasOBONamespace>GAZ</oboInOwl:hasOBONamespace>
        <oboInOwl:id>GAZ:00058463</oboInOwl:id>
        <rdfs:label>Deosai National Park</rdfs:label>
    </owl:NamedIndividual>
    


    <!-- http://purl.obolibrary.org/obo/GAZ_00058464 -->

    <owl:NamedIndividual rdf:about="http://purl.obolibrary.org/obo/GAZ_00058464">
        <obo:RO_0001025 rdf:resource="http://purl.obolibrary.org/obo/GAZ_00058463"/>
        <obo:IAO_0000115>A lake situated in Deosai Plains, Northern Areas of Pakistan.</obo:IAO_0000115>
        <oboInOwl:hasOBONamespace>GAZ</oboInOwl:hasOBONamespace>
        <oboInOwl:id>GAZ:00058464</oboInOwl:id>
        <rdfs:label>Sheosar Lake</rdfs:label>
    </owl:NamedIndividual>
    


    <!-- http://purl.obolibrary.org/obo/GAZ_00058465 -->

    <owl:NamedIndividual rdf:about="http://purl.obolibrary.org/obo/GAZ_00058465">
        <obo:RO_0001025 rdf:resource="http://purl.obolibrary.org/obo/GAZ_00400020"/>
        <obo:IAO_0000115>A brackish lake. Located near the Karachi to Uthal road, 90 km NNW of Karachi, Lasbella District, Baluchistan Province.</obo:IAO_0000115>
        <oboInOwl:hasOBONamespace>GAZ</oboInOwl:hasOBONamespace>
        <oboInOwl:id>GAZ:00058465</oboInOwl:id>
        <rdfs:label>Siranda Lake</rdfs:label>
    </owl:NamedIndividual>
    


    <!-- http://purl.obolibrary.org/obo/GAZ_00058466 -->

    <owl:NamedIndividual rdf:about="http://purl.obolibrary.org/obo/GAZ_00058466">
        <obo:RO_0001025 rdf:resource="http://purl.obolibrary.org/obo/GAZ_00005246"/>
        <oboInOwl:hasOBONamespace>GAZ</oboInOwl:hasOBONamespace>
        <oboInOwl:id>GAZ:00058466</oboInOwl:id>
        <rdfs:label>Jhelum Valley</rdfs:label>
    </owl:NamedIndividual>
    


    <!-- http://purl.obolibrary.org/obo/GAZ_00058467 -->

    <owl:NamedIndividual rdf:about="http://purl.obolibrary.org/obo/GAZ_00058467">
        <obo:RO_0001025 rdf:resource="http://purl.obolibrary.org/obo/GAZ_00058466"/>
        <obo:IAO_0000115>The largest and most western of the five rivers of Punjab, and passes through Jhelum District. It is a tributary of the Indus River and has a total length of about 772 km. The river Jhelum rises from a spring at Verinag situated at the foot of the Pir Panjal in the south-eastern part of the valley of Kashmir. It flows through Srinagar and the Wular lake before entering Pakistan through a deep narrow gorge. The Kishenganga (Neelum) River, the largest tributary of the Jhelum, joins it near Muzaffarabad, as does the next largest, the Kunhar River of the Kaghan valley. It also connects with Pakistan and Pakistan-held Kashmir on Kohala Bridge east of Circle Bakote. It is then joined by the Poonch river, and flows into the Mangla Dam reservoir in the district of Mirpur. The Jhelum enters the Punjab in the Jhelum District. From there, it flows through the plains of Pakistan&apos;s Punjab, forming the boundary between the Chaj and Sindh Sagar Doabs. It ends in a confluence with the Chenab at Trimmu in District Jhang. The Chenab merges with the Sutlej to form the Panjnad River which joins the Indus River at Mithankot.</obo:IAO_0000115>
        <oboInOwl:hasOBONamespace>GAZ</oboInOwl:hasOBONamespace>
        <oboInOwl:id>GAZ:00058467</oboInOwl:id>
        <rdfs:label>Jhelum River</rdfs:label>
    </owl:NamedIndividual>
    


    <!-- http://purl.obolibrary.org/obo/GAZ_00058468 -->

    <owl:NamedIndividual rdf:about="http://purl.obolibrary.org/obo/GAZ_00058468">
        <obo:RO_0001025 rdf:resource="http://purl.obolibrary.org/obo/GAZ_00005257"/>
        <obo:RO_0001025 rdf:resource="http://purl.obolibrary.org/obo/GAZ_00058467"/>
        <obo:IAO_0000115>A lake.</obo:IAO_0000115>
        <oboInOwl:hasOBONamespace>GAZ</oboInOwl:hasOBONamespace>
        <oboInOwl:id>GAZ:00058468</oboInOwl:id>
        <rdfs:label>Subri Lake</rdfs:label>
    </owl:NamedIndividual>
    


    <!-- http://purl.obolibrary.org/obo/GAZ_00058469 -->

    <owl:NamedIndividual rdf:about="http://purl.obolibrary.org/obo/GAZ_00058469">
        <obo:RO_0001025 rdf:resource="http://purl.obolibrary.org/obo/GAZ_00018568"/>
        <obo:IAO_0000115>A lake situated at 975 m above sea-level in the Samahni valley, Mirpur District.</obo:IAO_0000115>
        <oboInOwl:hasOBONamespace>GAZ</oboInOwl:hasOBONamespace>
        <oboInOwl:id>GAZ:00058469</oboInOwl:id>
        <rdfs:label>Baghsar Lake</rdfs:label>
    </owl:NamedIndividual>
    


    <!-- http://purl.obolibrary.org/obo/GAZ_00058470 -->

    <owl:NamedIndividual rdf:about="http://purl.obolibrary.org/obo/GAZ_00058470">
        <obo:RO_0001025 rdf:resource="http://purl.obolibrary.org/obo/GAZ_00253151"/>
        <obo:IAO_0000115>A brackish lake located in Thatta District, Sindh, Pakistan.</obo:IAO_0000115>
        <oboInOwl:hasOBONamespace>GAZ</oboInOwl:hasOBONamespace>
        <oboInOwl:id>GAZ:00058470</oboInOwl:id>
        <rdfs:label>Hadero Lake</rdfs:label>
    </owl:NamedIndividual>
    


    <!-- http://purl.obolibrary.org/obo/GAZ_00058471 -->

    <owl:NamedIndividual rdf:about="http://purl.obolibrary.org/obo/GAZ_00058471">
        <obo:RO_0001025 rdf:resource="http://purl.obolibrary.org/obo/GAZ_00253070"/>
        <obo:IAO_0000115>A saline lake in the southern Salt Range area in Pakistan.</obo:IAO_0000115>
        <oboInOwl:hasOBONamespace>GAZ</oboInOwl:hasOBONamespace>
        <oboInOwl:id>GAZ:00058471</oboInOwl:id>
        <rdfs:label>Khabikki Lake</rdfs:label>
    </owl:NamedIndividual>
    


    <!-- http://purl.obolibrary.org/obo/GAZ_00058472 -->

    <owl:NamedIndividual rdf:about="http://purl.obolibrary.org/obo/GAZ_00058472">
        <obo:RO_0001025 rdf:resource="http://purl.obolibrary.org/obo/GAZ_00058423"/>
        <obo:IAO_0000115>A lake located near Shogran in the Kaghan Valley in Pakistan.</obo:IAO_0000115>
        <oboInOwl:hasOBONamespace>GAZ</oboInOwl:hasOBONamespace>
        <oboInOwl:id>GAZ:00058472</oboInOwl:id>
        <rdfs:label>Payee Lake</rdfs:label>
    </owl:NamedIndividual>
    


    <!-- http://purl.obolibrary.org/obo/GAZ_00058473 -->

    <owl:NamedIndividual rdf:about="http://purl.obolibrary.org/obo/GAZ_00058473">
        <obo:RO_0001025 rdf:resource="http://purl.obolibrary.org/obo/GAZ_00400049"/>
    </owl:NamedIndividual>
    


    <!-- http://purl.obolibrary.org/obo/GAZ_00058474 -->

    <owl:NamedIndividual rdf:about="http://purl.obolibrary.org/obo/GAZ_00058474">
        <obo:RO_0001025 rdf:resource="http://purl.obolibrary.org/obo/GAZ_00058475"/>
        <obo:IAO_0000115>A rectangular natural lake on the Elum Ghar mountain in Pir Baba, Buner District, North-West Frontier Province, Pakistan.</obo:IAO_0000115>
        <oboInOwl:hasOBONamespace>GAZ</oboInOwl:hasOBONamespace>
        <oboInOwl:id>GAZ:00058474</oboInOwl:id>
        <rdfs:label>Peryano Dand</rdfs:label>
    </owl:NamedIndividual>
    


    <!-- http://purl.obolibrary.org/obo/GAZ_00058475 -->

    <owl:NamedIndividual rdf:about="http://purl.obolibrary.org/obo/GAZ_00058475">
        <obo:RO_0001025 rdf:resource="http://purl.obolibrary.org/obo/GAZ_00058473"/>
        <obo:IAO_0000115>A mountain of Pir Baba in the Buner District of the North-West Frontier Province of Pakistan. It lies on the westside of Pir Baba. Its height is approximately 2,800 m.</obo:IAO_0000115>
        <oboInOwl:hasOBONamespace>GAZ</oboInOwl:hasOBONamespace>
        <oboInOwl:id>GAZ:00058475</oboInOwl:id>
        <rdfs:label>Elum Ghar</rdfs:label>
    </owl:NamedIndividual>
    


    <!-- http://purl.obolibrary.org/obo/GAZ_00058476 -->

    <owl:NamedIndividual rdf:about="http://purl.obolibrary.org/obo/GAZ_00058476">
        <obo:RO_0001025 rdf:resource="http://purl.obolibrary.org/obo/GAZ_00058477"/>
        <obo:IAO_0000115>A saline lake in Soan Sakaser Valley in the southern Salt Range area in Pakistan.</obo:IAO_0000115>
        <oboInOwl:hasOBONamespace>GAZ</oboInOwl:hasOBONamespace>
        <oboInOwl:id>GAZ:00058476</oboInOwl:id>
        <rdfs:label>Uchhali Lake</rdfs:label>
    </owl:NamedIndividual>
    


    <!-- http://purl.obolibrary.org/obo/GAZ_00058477 -->

    <owl:NamedIndividual rdf:about="http://purl.obolibrary.org/obo/GAZ_00058477">
        <obo:RO_0001025 rdf:resource="http://purl.obolibrary.org/obo/GAZ_00056904"/>
        <obo:IAO_0000115>A valley situated in northern Punjab, Pakistan. Soan Sakaser is situated on the juncture Mianwali, Khushab and Chakwal districts. On the north of this valley is Tehsil Tala Gang&apos;s area Pakhar; on the east side is tehsil Chakwal&apos;s area Venhar; on the south side hilly area of tehsil Khushab; and on east side, Mianwal tehsil are situated.</obo:IAO_0000115>
        <oboInOwl:hasOBONamespace>GAZ</oboInOwl:hasOBONamespace>
        <oboInOwl:id>GAZ:00058477</oboInOwl:id>
        <rdfs:label>Soan Sakaser Valley</rdfs:label>
    </owl:NamedIndividual>
    


    <!-- http://purl.obolibrary.org/obo/GAZ_00058498 -->

    <owl:NamedIndividual rdf:about="http://purl.obolibrary.org/obo/GAZ_00058498">
        <obo:RO_0001025 rdf:resource="http://purl.obolibrary.org/obo/GAZ_00004988"/>
        <obo:IAO_0000115>A 25 km diameter crater lake in the Pamir Mountains in Tajikistan, which lies at an altitude of 3,900 meters (13,000 feet) above mean sea level. A peninsula projecting from the south shore and an island off the north shore divide the lake into two basins, a smaller eastern one which is relatively shallow, between 13 to 19 meters, and a larger western one, with depths of 221 to 230 meters. It has no drainage outlet. Kara-Kul lake lies within a circular depression interpreted as a meteorite impact crater with a rim diameter of 45 km.</obo:IAO_0000115>
        <oboInOwl:hasOBONamespace>GAZ</oboInOwl:hasOBONamespace>
        <oboInOwl:id>GAZ:00058498</oboInOwl:id>
        <rdfs:label>Kara-Kul</rdfs:label>
    </owl:NamedIndividual>
    


    <!-- http://purl.obolibrary.org/obo/GAZ_00058499 -->

    <owl:NamedIndividual rdf:about="http://purl.obolibrary.org/obo/GAZ_00058499">
        <obo:RO_0001025 rdf:resource="http://purl.obolibrary.org/obo/GAZ_00004988"/>
        <obo:IAO_0000115>A lake in Tajikistan, in the northeast Pamir Mountains, northwest of the Muztagh Ata peak (7,880 metres), at an altitude of 3,870 m. It is a moraine lake; and a stream of the same name flows through it.</obo:IAO_0000115>
        <oboInOwl:hasOBONamespace>GAZ</oboInOwl:hasOBONamespace>
        <oboInOwl:id>GAZ:00058499</oboInOwl:id>
        <rdfs:label>Little Kara-Kul</rdfs:label>
    </owl:NamedIndividual>
    


    <!-- http://purl.obolibrary.org/obo/GAZ_00058502 -->

    <owl:NamedIndividual rdf:about="http://purl.obolibrary.org/obo/GAZ_00058502">
        <obo:RO_0001025 rdf:resource="http://purl.obolibrary.org/obo/GAZ_00004988"/>
        <obo:IAO_0000115>A lake in Pamir, Tajikistan. The lake formed in 1911, after a great earthquake, when the Murghab River was blocked by a big landslide, forming the Usoi Dam.</obo:IAO_0000115>
        <oboInOwl:hasOBONamespace>GAZ</oboInOwl:hasOBONamespace>
        <oboInOwl:id>GAZ:00058502</oboInOwl:id>
        <rdfs:label>Sarez Lake</rdfs:label>
    </owl:NamedIndividual>
    


    <!-- http://purl.obolibrary.org/obo/GAZ_00058503 -->

    <owl:NamedIndividual rdf:about="http://purl.obolibrary.org/obo/GAZ_00058503">
        <obo:RO_0001025 rdf:resource="http://purl.obolibrary.org/obo/GAZ_00004988"/>
        <obo:IAO_0000115>A natural landslide dam along the Murghab River in the Central Asian nation of Tajikistan. Established 1911-02-18, when a great earthquake estimated between 8 and 9 on the Richter Scale caused a massive landslide to block the flow of the river.</obo:IAO_0000115>
        <oboInOwl:hasOBONamespace>GAZ</oboInOwl:hasOBONamespace>
        <oboInOwl:id>GAZ:00058503</oboInOwl:id>
        <rdfs:label>Usoi Dam</rdfs:label>
    </owl:NamedIndividual>
    


    <!-- http://purl.obolibrary.org/obo/GAZ_00080147 -->

    <owl:NamedIndividual rdf:about="http://purl.obolibrary.org/obo/GAZ_00080147">
        <obo:RO_0001025 rdf:resource="http://purl.obolibrary.org/obo/GAZ_00018488"/>
        <obo:RO_0001025 rdf:resource="http://purl.obolibrary.org/obo/GAZ_00400020"/>
        <obo:IAO_0000115>A national park that covers about 1,650 km2 and is the largest of National Parks of Pakistan and lies on the Makran coast in Balochistan and approximately 190 km from Karachi. The area was for the first time declared reserved in 1988.</obo:IAO_0000115>
        <oboInOwl:hasOBONamespace>GAZ</oboInOwl:hasOBONamespace>
        <oboInOwl:id>GAZ:00080147</oboInOwl:id>
        <rdfs:label>Hingol National Park</rdfs:label>
    </owl:NamedIndividual>
    


    <!-- http://purl.obolibrary.org/obo/GAZ_00080149 -->

    <owl:NamedIndividual rdf:about="http://purl.obolibrary.org/obo/GAZ_00080149">
        <obo:RO_0001025 rdf:resource="http://purl.obolibrary.org/obo/GAZ_00018583"/>
        <obo:IAO_0000115>A national park in the Northern Areas of Pakistan. It is one of the highest altitude parks in the world.</obo:IAO_0000115>
        <oboInOwl:hasOBONamespace>GAZ</oboInOwl:hasOBONamespace>
        <oboInOwl:id>GAZ:00080149</oboInOwl:id>
        <rdfs:label>Khunjerab National Park</rdfs:label>
    </owl:NamedIndividual>
    


    <!-- http://purl.obolibrary.org/obo/GAZ_00080150 -->

    <owl:NamedIndividual rdf:about="http://purl.obolibrary.org/obo/GAZ_00080150">
        <obo:RO_0001025 rdf:resource="http://purl.obolibrary.org/obo/GAZ_00400045"/>
        <obo:IAO_0000115>A national park.</obo:IAO_0000115>
        <oboInOwl:hasOBONamespace>GAZ</oboInOwl:hasOBONamespace>
        <oboInOwl:id>GAZ:00080150</oboInOwl:id>
        <rdfs:label>Chitral Gol National Park</rdfs:label>
    </owl:NamedIndividual>
    


    <!-- http://purl.obolibrary.org/obo/GAZ_00080151 -->

    <owl:NamedIndividual rdf:about="http://purl.obolibrary.org/obo/GAZ_00080151">
        <obo:RO_0001025 rdf:resource="http://purl.obolibrary.org/obo/GAZ_00400077"/>
        <obo:IAO_0000115>A national park.</obo:IAO_0000115>
        <oboInOwl:hasOBONamespace>GAZ</oboInOwl:hasOBONamespace>
        <oboInOwl:id>GAZ:00080151</oboInOwl:id>
        <rdfs:label>Lal Suhanra National Park</rdfs:label>
    </owl:NamedIndividual>
    


    <!-- http://purl.obolibrary.org/obo/GAZ_00080152 -->

    <owl:NamedIndividual rdf:about="http://purl.obolibrary.org/obo/GAZ_00080152">
        <obo:RO_0001025 rdf:resource="http://purl.obolibrary.org/obo/GAZ_00400006"/>
        <obo:IAO_0000115>A national park located 20 km south-west of Quetta.</obo:IAO_0000115>
        <oboInOwl:hasOBONamespace>GAZ</oboInOwl:hasOBONamespace>
        <oboInOwl:id>GAZ:00080152</oboInOwl:id>
        <rdfs:label>Hazarganji-Chiltan National Park</rdfs:label>
    </owl:NamedIndividual>
    


    <!-- http://purl.obolibrary.org/obo/GAZ_00080153 -->

    <owl:NamedIndividual rdf:about="http://purl.obolibrary.org/obo/GAZ_00080153">
        <obo:RO_0001025 rdf:resource="http://purl.obolibrary.org/obo/GAZ_00005250"/>
        <obo:IAO_0000115>A national park in NWFP, Pakistan. It is a small natural park located at 26 km from the Murree hill station.</obo:IAO_0000115>
        <oboInOwl:hasOBONamespace>GAZ</oboInOwl:hasOBONamespace>
        <oboInOwl:id>GAZ:00080153</oboInOwl:id>
        <rdfs:label>Ayubia National Park</rdfs:label>
    </owl:NamedIndividual>
    


    <!-- http://purl.obolibrary.org/obo/GAZ_00080154 -->

    <owl:NamedIndividual rdf:about="http://purl.obolibrary.org/obo/GAZ_00080154">
        <obo:RO_0001025 rdf:resource="http://purl.obolibrary.org/obo/GAZ_00400073"/>
        <obo:IAO_0000115>A protected area in Jhelum District, northern Punjab, Pakistan. The park is almost 90 km on GT Road in the hilly Pothohar region from Islamabad. It is 10 km from GT Road.</obo:IAO_0000115>
        <oboInOwl:hasOBONamespace>GAZ</oboInOwl:hasOBONamespace>
        <oboInOwl:id>GAZ:00080154</oboInOwl:id>
        <rdfs:label>Lehri Nature Park</rdfs:label>
    </owl:NamedIndividual>
    


    <!-- http://purl.obolibrary.org/obo/GAZ_00080155 -->

    <owl:NamedIndividual rdf:about="http://purl.obolibrary.org/obo/GAZ_00080155">
        <obo:RO_0001025 rdf:resource="http://purl.obolibrary.org/obo/GAZ_00005246"/>
        <obo:IAO_0000115>A national park in Pakistan.</obo:IAO_0000115>
        <oboInOwl:hasOBONamespace>GAZ</oboInOwl:hasOBONamespace>
        <oboInOwl:id>GAZ:00080155</oboInOwl:id>
        <rdfs:label>Machiara National Park</rdfs:label>
    </owl:NamedIndividual>
    


    <!-- http://purl.obolibrary.org/obo/GAZ_00080156 -->

    <owl:NamedIndividual rdf:about="http://purl.obolibrary.org/obo/GAZ_00080156">
        <obo:RO_0001025 rdf:resource="http://purl.obolibrary.org/obo/GAZ_00005246"/>
        <obo:IAO_0000115>A national park in Pakistan.</obo:IAO_0000115>
        <oboInOwl:hasOBONamespace>GAZ</oboInOwl:hasOBONamespace>
        <oboInOwl:id>GAZ:00080156</oboInOwl:id>
        <rdfs:label>Toh Pir National Park</rdfs:label>
    </owl:NamedIndividual>
    


    <!-- http://purl.obolibrary.org/obo/GAZ_00080157 -->

    <owl:NamedIndividual rdf:about="http://purl.obolibrary.org/obo/GAZ_00080157">
        <obo:RO_0001025 rdf:resource="http://purl.obolibrary.org/obo/GAZ_00005246"/>
        <obo:IAO_0000115>A national park in Pakistan.</obo:IAO_0000115>
        <oboInOwl:hasOBONamespace>GAZ</oboInOwl:hasOBONamespace>
        <oboInOwl:id>GAZ:00080157</oboInOwl:id>
        <rdfs:label>Gamot National Park</rdfs:label>
    </owl:NamedIndividual>
    


    <!-- http://purl.obolibrary.org/obo/GAZ_00080158 -->

    <owl:NamedIndividual rdf:about="http://purl.obolibrary.org/obo/GAZ_00080158">
        <obo:RO_0001025 rdf:resource="http://purl.obolibrary.org/obo/GAZ_00005246"/>
        <obo:IAO_0000115>A national park in Pakistan.</obo:IAO_0000115>
        <oboInOwl:hasOBONamespace>GAZ</oboInOwl:hasOBONamespace>
        <oboInOwl:id>GAZ:00080158</oboInOwl:id>
        <rdfs:label>Pir Lasoora National Park</rdfs:label>
    </owl:NamedIndividual>
    


    <!-- http://purl.obolibrary.org/obo/GAZ_00080159 -->

    <owl:NamedIndividual rdf:about="http://purl.obolibrary.org/obo/GAZ_00080159">
        <obo:RO_0001025 rdf:resource="http://purl.obolibrary.org/obo/GAZ_00005246"/>
        <obo:IAO_0000115>A national park in Pakistan.</obo:IAO_0000115>
        <oboInOwl:hasOBONamespace>GAZ</oboInOwl:hasOBONamespace>
        <oboInOwl:id>GAZ:00080159</oboInOwl:id>
        <rdfs:label>Chinji National Park</rdfs:label>
    </owl:NamedIndividual>
    


    <!-- http://purl.obolibrary.org/obo/GAZ_00080160 -->

    <owl:NamedIndividual rdf:about="http://purl.obolibrary.org/obo/GAZ_00080160">
        <obo:RO_0001025 rdf:resource="http://purl.obolibrary.org/obo/GAZ_00005246"/>
        <obo:IAO_0000115>A national park in Pakistan.</obo:IAO_0000115>
        <oboInOwl:hasOBONamespace>GAZ</oboInOwl:hasOBONamespace>
        <oboInOwl:id>GAZ:00080160</oboInOwl:id>
        <rdfs:label>Handrap-Shandoor National Park</rdfs:label>
    </owl:NamedIndividual>
    


    <!-- http://purl.obolibrary.org/obo/GAZ_00080161 -->

    <owl:NamedIndividual rdf:about="http://purl.obolibrary.org/obo/GAZ_00080161">
        <obo:RO_0001025 rdf:resource="http://purl.obolibrary.org/obo/GAZ_00005246"/>
        <obo:IAO_0000115>A national park in Pakistan.</obo:IAO_0000115>
        <oboInOwl:hasOBONamespace>GAZ</oboInOwl:hasOBONamespace>
        <oboInOwl:id>GAZ:00080161</oboInOwl:id>
        <rdfs:label>Saiful Malook National Park</rdfs:label>
    </owl:NamedIndividual>
    


    <!-- http://purl.obolibrary.org/obo/GAZ_00080162 -->

    <owl:NamedIndividual rdf:about="http://purl.obolibrary.org/obo/GAZ_00080162">
        <obo:RO_0001025 rdf:resource="http://purl.obolibrary.org/obo/GAZ_00005246"/>
        <obo:IAO_0000115>A national park in Pakistan.</obo:IAO_0000115>
        <oboInOwl:hasOBONamespace>GAZ</oboInOwl:hasOBONamespace>
        <oboInOwl:id>GAZ:00080162</oboInOwl:id>
        <rdfs:label>Sheikh Badin National Park</rdfs:label>
    </owl:NamedIndividual>
    


    <!-- http://purl.obolibrary.org/obo/GAZ_00080163 -->

    <owl:NamedIndividual rdf:about="http://purl.obolibrary.org/obo/GAZ_00080163">
        <obo:RO_0001025 rdf:resource="http://purl.obolibrary.org/obo/GAZ_00005246"/>
        <obo:IAO_0000115>A national park in Pakistan.</obo:IAO_0000115>
        <oboInOwl:hasOBONamespace>GAZ</oboInOwl:hasOBONamespace>
        <oboInOwl:id>GAZ:00080163</oboInOwl:id>
        <rdfs:label>Lulusar-Dodipat National Park</rdfs:label>
    </owl:NamedIndividual>
    


    <!-- http://purl.obolibrary.org/obo/GAZ_00080164 -->

    <owl:NamedIndividual rdf:about="http://purl.obolibrary.org/obo/GAZ_00080164">
        <obo:RO_0001025 rdf:resource="http://purl.obolibrary.org/obo/GAZ_00018580"/>
        <obo:RO_0001025 rdf:resource="http://purl.obolibrary.org/obo/GAZ_00018583"/>
        <obo:IAO_0000115>A national park in the Northern Areas of Pakistan that comprises the Baltoro, Panmah, Biafo and Hispar glaciers and their tributary glaciers. The Central Karakoram National Park lies mostly in Skardu District of the Northern Areas, but also includes area within the Gilgit District.</obo:IAO_0000115>
        <oboInOwl:hasOBONamespace>GAZ</oboInOwl:hasOBONamespace>
        <oboInOwl:id>GAZ:00080164</oboInOwl:id>
        <rdfs:label>Central Karakoram National Park</rdfs:label>
    </owl:NamedIndividual>
    


    <!-- http://purl.obolibrary.org/obo/GAZ_00080165 -->

    <owl:NamedIndividual rdf:about="http://purl.obolibrary.org/obo/GAZ_00080165">
        <obo:RO_0001025 rdf:resource="http://purl.obolibrary.org/obo/GAZ_00400008"/>
        <obo:IAO_0000115>One of the 4 Tehsils of Awaran District, Balochistan.</obo:IAO_0000115>
        <oboInOwl:hasOBONamespace>GAZ</oboInOwl:hasOBONamespace>
        <oboInOwl:id>GAZ:00080165</oboInOwl:id>
        <rdfs:label>Mashkay Tehsil</rdfs:label>
    </owl:NamedIndividual>
    


    <!-- http://purl.obolibrary.org/obo/GAZ_00080166 -->

    <owl:NamedIndividual rdf:about="http://purl.obolibrary.org/obo/GAZ_00080166">
        <obo:RO_0001025 rdf:resource="http://purl.obolibrary.org/obo/GAZ_00400008"/>
        <obo:IAO_0000115>One of the 4 Tehsils of Awaran District, Balochistan.</obo:IAO_0000115>
        <oboInOwl:hasOBONamespace>GAZ</oboInOwl:hasOBONamespace>
        <oboInOwl:id>GAZ:00080166</oboInOwl:id>
        <rdfs:label>Awaran Tehsil</rdfs:label>
    </owl:NamedIndividual>
    


    <!-- http://purl.obolibrary.org/obo/GAZ_00080167 -->

    <owl:NamedIndividual rdf:about="http://purl.obolibrary.org/obo/GAZ_00080167">
        <obo:RO_0001025 rdf:resource="http://purl.obolibrary.org/obo/GAZ_00400008"/>
        <obo:IAO_0000115>One of the 4 Tehsils of Awaran District, Balochistan.</obo:IAO_0000115>
        <oboInOwl:hasOBONamespace>GAZ</oboInOwl:hasOBONamespace>
        <oboInOwl:id>GAZ:00080167</oboInOwl:id>
        <rdfs:label>Gashkore Tehsil</rdfs:label>
    </owl:NamedIndividual>
    


    <!-- http://purl.obolibrary.org/obo/GAZ_00080168 -->

    <owl:NamedIndividual rdf:about="http://purl.obolibrary.org/obo/GAZ_00080168">
        <obo:RO_0001025 rdf:resource="http://purl.obolibrary.org/obo/GAZ_00400008"/>
        <obo:IAO_0000115>One of the 4 Tehsils of Awaran District, Balochistan.</obo:IAO_0000115>
        <oboInOwl:hasOBONamespace>GAZ</oboInOwl:hasOBONamespace>
        <oboInOwl:id>GAZ:00080168</oboInOwl:id>
        <rdfs:label>Jhal Jhao Tehsil</rdfs:label>
    </owl:NamedIndividual>
    


    <!-- http://purl.obolibrary.org/obo/GAZ_00080169 -->

    <owl:NamedIndividual rdf:about="http://purl.obolibrary.org/obo/GAZ_00080169">
        <obo:RO_0001025 rdf:resource="http://purl.obolibrary.org/obo/GAZ_00400003"/>
        <obo:IAO_0000115>The only Tehsils of Barkhan District, Balochistan.</obo:IAO_0000115>
        <oboInOwl:hasOBONamespace>GAZ</oboInOwl:hasOBONamespace>
        <oboInOwl:id>GAZ:00080169</oboInOwl:id>
        <rdfs:label>Barkhan Tehsil</rdfs:label>
    </owl:NamedIndividual>
    


    <!-- http://purl.obolibrary.org/obo/GAZ_00080170 -->

    <owl:NamedIndividual rdf:about="http://purl.obolibrary.org/obo/GAZ_00080170">
        <obo:RO_0001025 rdf:resource="http://purl.obolibrary.org/obo/GAZ_00400007"/>
        <obo:IAO_0000115>One of the 6 Tehsils of Bolan District, Balochistan.</obo:IAO_0000115>
        <oboInOwl:hasOBONamespace>GAZ</oboInOwl:hasOBONamespace>
        <oboInOwl:id>GAZ:00080170</oboInOwl:id>
        <rdfs:label>Khattan Tehsil</rdfs:label>
    </owl:NamedIndividual>
    


    <!-- http://purl.obolibrary.org/obo/GAZ_00080171 -->

    <owl:NamedIndividual rdf:about="http://purl.obolibrary.org/obo/GAZ_00080171">
        <obo:RO_0001025 rdf:resource="http://purl.obolibrary.org/obo/GAZ_00400007"/>
        <obo:IAO_0000115>One of the 6 Tehsils of Bolan District, Balochistan.</obo:IAO_0000115>
        <oboInOwl:hasOBONamespace>GAZ</oboInOwl:hasOBONamespace>
        <oboInOwl:id>GAZ:00080171</oboInOwl:id>
        <rdfs:label>Bhag Tehsil</rdfs:label>
    </owl:NamedIndividual>
    


    <!-- http://purl.obolibrary.org/obo/GAZ_00080172 -->

    <owl:NamedIndividual rdf:about="http://purl.obolibrary.org/obo/GAZ_00080172">
        <obo:RO_0001025 rdf:resource="http://purl.obolibrary.org/obo/GAZ_00400007"/>
        <obo:IAO_0000115>One of the 6 Tehsils of Bolan District, Balochistan.</obo:IAO_0000115>
        <oboInOwl:hasOBONamespace>GAZ</oboInOwl:hasOBONamespace>
        <oboInOwl:id>GAZ:00080172</oboInOwl:id>
        <rdfs:label>Sani Tehsil</rdfs:label>
    </owl:NamedIndividual>
    


    <!-- http://purl.obolibrary.org/obo/GAZ_00080173 -->

    <owl:NamedIndividual rdf:about="http://purl.obolibrary.org/obo/GAZ_00080173">
        <obo:RO_0001025 rdf:resource="http://purl.obolibrary.org/obo/GAZ_00400007"/>
        <obo:IAO_0000115>One of the 6 Tehsils of Bolan District, Balochistan.</obo:IAO_0000115>
        <oboInOwl:hasOBONamespace>GAZ</oboInOwl:hasOBONamespace>
        <oboInOwl:id>GAZ:00080173</oboInOwl:id>
        <rdfs:label>Dhadar Tehsil</rdfs:label>
    </owl:NamedIndividual>
    


    <!-- http://purl.obolibrary.org/obo/GAZ_00080174 -->

    <owl:NamedIndividual rdf:about="http://purl.obolibrary.org/obo/GAZ_00080174">
        <obo:RO_0001025 rdf:resource="http://purl.obolibrary.org/obo/GAZ_00400007"/>
        <obo:IAO_0000115>One of the 6 Tehsils of Bolan District, Balochistan.</obo:IAO_0000115>
        <oboInOwl:hasOBONamespace>GAZ</oboInOwl:hasOBONamespace>
        <oboInOwl:id>GAZ:00080174</oboInOwl:id>
        <rdfs:label>Balanari Tehsil</rdfs:label>
    </owl:NamedIndividual>
    


    <!-- http://purl.obolibrary.org/obo/GAZ_00080175 -->

    <owl:NamedIndividual rdf:about="http://purl.obolibrary.org/obo/GAZ_00080175">
        <obo:RO_0001025 rdf:resource="http://purl.obolibrary.org/obo/GAZ_00400007"/>
        <obo:IAO_0000115>One of the 6 Tehsils of Bolan District, Balochistan.</obo:IAO_0000115>
        <oboInOwl:hasOBONamespace>GAZ</oboInOwl:hasOBONamespace>
        <oboInOwl:id>GAZ:00080175</oboInOwl:id>
        <rdfs:label>Mach Tehsil</rdfs:label>
    </owl:NamedIndividual>
    


    <!-- http://purl.obolibrary.org/obo/GAZ_00080176 -->

    <owl:NamedIndividual rdf:about="http://purl.obolibrary.org/obo/GAZ_00080176">
        <obo:RO_0001025 rdf:resource="http://purl.obolibrary.org/obo/GAZ_00400004"/>
        <obo:IAO_0000115>One of the 2 Tehsils of Nushki District, Balochistan.</obo:IAO_0000115>
        <oboInOwl:hasOBONamespace>GAZ</oboInOwl:hasOBONamespace>
        <oboInOwl:id>GAZ:00080176</oboInOwl:id>
        <rdfs:label>Dalbandin Tehsil</rdfs:label>
    </owl:NamedIndividual>
    


    <!-- http://purl.obolibrary.org/obo/GAZ_00080177 -->

    <owl:NamedIndividual rdf:about="http://purl.obolibrary.org/obo/GAZ_00080177">
        <obo:RO_0001025 rdf:resource="http://purl.obolibrary.org/obo/GAZ_00400004"/>
        <obo:IAO_0000115>One of the 2 Tehsils of Nushki District, Balochistan.</obo:IAO_0000115>
        <oboInOwl:hasOBONamespace>GAZ</oboInOwl:hasOBONamespace>
        <oboInOwl:id>GAZ:00080177</oboInOwl:id>
        <rdfs:label>Nushki Tehsil</rdfs:label>
    </owl:NamedIndividual>
    


    <!-- http://purl.obolibrary.org/obo/GAZ_00080178 -->

    <owl:NamedIndividual rdf:about="http://purl.obolibrary.org/obo/GAZ_00080178">
        <obo:RO_0001025 rdf:resource="http://purl.obolibrary.org/obo/GAZ_00400000"/>
        <obo:IAO_0000115>One of the 4 Tehsils of Chagai District, Balochistan.</obo:IAO_0000115>
        <oboInOwl:hasOBONamespace>GAZ</oboInOwl:hasOBONamespace>
        <oboInOwl:id>GAZ:00080178</oboInOwl:id>
        <rdfs:label>Chagai Tehsil</rdfs:label>
    </owl:NamedIndividual>
    


    <!-- http://purl.obolibrary.org/obo/GAZ_00080179 -->

    <owl:NamedIndividual rdf:about="http://purl.obolibrary.org/obo/GAZ_00080179">
        <obo:RO_0001025 rdf:resource="http://purl.obolibrary.org/obo/GAZ_00400000"/>
        <obo:IAO_0000115>One of the 4 Tehsils of Chagai District, Balochistan.</obo:IAO_0000115>
        <oboInOwl:hasOBONamespace>GAZ</oboInOwl:hasOBONamespace>
        <oboInOwl:id>GAZ:00080179</oboInOwl:id>
        <rdfs:label>Nokundi Tehsil</rdfs:label>
    </owl:NamedIndividual>
    


    <!-- http://purl.obolibrary.org/obo/GAZ_00080180 -->

    <owl:NamedIndividual rdf:about="http://purl.obolibrary.org/obo/GAZ_00080180">
        <obo:RO_0001025 rdf:resource="http://purl.obolibrary.org/obo/GAZ_00400000"/>
        <obo:IAO_0000115>One of the 4 Tehsils of Chagai District, Balochistan.</obo:IAO_0000115>
        <oboInOwl:hasOBONamespace>GAZ</oboInOwl:hasOBONamespace>
        <oboInOwl:id>GAZ:00080180</oboInOwl:id>
        <rdfs:label>Taftan Tehsil</rdfs:label>
    </owl:NamedIndividual>
    


    <!-- http://purl.obolibrary.org/obo/GAZ_00080181 -->

    <owl:NamedIndividual rdf:about="http://purl.obolibrary.org/obo/GAZ_00080181">
        <obo:RO_0001025 rdf:resource="http://purl.obolibrary.org/obo/GAZ_00400000"/>
        <obo:IAO_0000115>One of the 4 Tehsils of Chagai District, Balochistan.</obo:IAO_0000115>
        <oboInOwl:hasOBONamespace>GAZ</oboInOwl:hasOBONamespace>
        <oboInOwl:id>GAZ:00080181</oboInOwl:id>
        <rdfs:label>Dak Tehsil</rdfs:label>
    </owl:NamedIndividual>
    


    <!-- http://purl.obolibrary.org/obo/GAZ_00080182 -->

    <owl:NamedIndividual rdf:about="http://purl.obolibrary.org/obo/GAZ_00080182">
        <obo:RO_0001025 rdf:resource="http://purl.obolibrary.org/obo/GAZ_00400006"/>
        <obo:IAO_0000115>One of the 2 Tehsils of Quetta District, Balochistan.</obo:IAO_0000115>
        <oboInOwl:hasOBONamespace>GAZ</oboInOwl:hasOBONamespace>
        <oboInOwl:id>GAZ:00080182</oboInOwl:id>
        <rdfs:label>Panjpai Tehsil</rdfs:label>
    </owl:NamedIndividual>
    


    <!-- http://purl.obolibrary.org/obo/GAZ_00080183 -->

    <owl:NamedIndividual rdf:about="http://purl.obolibrary.org/obo/GAZ_00080183">
        <obo:RO_0001025 rdf:resource="http://purl.obolibrary.org/obo/GAZ_00400006"/>
        <obo:IAO_0000115>One of the 2 Tehsils of Quetta District, Balochistan.</obo:IAO_0000115>
        <oboInOwl:hasOBONamespace>GAZ</oboInOwl:hasOBONamespace>
        <oboInOwl:id>GAZ:00080183</oboInOwl:id>
        <rdfs:label>Quetta Tehsil</rdfs:label>
    </owl:NamedIndividual>
    


    <!-- http://purl.obolibrary.org/obo/GAZ_00080184 -->

    <owl:NamedIndividual rdf:about="http://purl.obolibrary.org/obo/GAZ_00080184">
        <obo:RO_0001025 rdf:resource="http://purl.obolibrary.org/obo/GAZ_00080183"/>
    </owl:NamedIndividual>
    


    <!-- http://purl.obolibrary.org/obo/GAZ_00080185 -->

    <owl:NamedIndividual rdf:about="http://purl.obolibrary.org/obo/GAZ_00080185">
        <obo:RO_0001025 rdf:resource="http://purl.obolibrary.org/obo/GAZ_00400021"/>
        <obo:IAO_0000115>A Tehsil of Dera Bugti District in the Balochistan province of Pakistan.</obo:IAO_0000115>
        <oboInOwl:hasOBONamespace>GAZ</oboInOwl:hasOBONamespace>
        <oboInOwl:id>GAZ:00080185</oboInOwl:id>
        <rdfs:label>Phelawagh Tehsil</rdfs:label>
    </owl:NamedIndividual>
    


    <!-- http://purl.obolibrary.org/obo/GAZ_00080186 -->

    <owl:NamedIndividual rdf:about="http://purl.obolibrary.org/obo/GAZ_00080186">
        <obo:RO_0001025 rdf:resource="http://purl.obolibrary.org/obo/GAZ_00400021"/>
        <obo:IAO_0000115>A Tehsil of Dera Bugti District in the Balochistan province of Pakistan.</obo:IAO_0000115>
        <oboInOwl:hasOBONamespace>GAZ</oboInOwl:hasOBONamespace>
        <oboInOwl:id>GAZ:00080186</oboInOwl:id>
        <rdfs:label>Sui Tehsil</rdfs:label>
    </owl:NamedIndividual>
    


    <!-- http://purl.obolibrary.org/obo/GAZ_00080187 -->

    <owl:NamedIndividual rdf:about="http://purl.obolibrary.org/obo/GAZ_00080187">
        <obo:RO_0001025 rdf:resource="http://purl.obolibrary.org/obo/GAZ_00400021"/>
        <obo:IAO_0000115>A Tehsil of Dera Bugti District in the Balochistan province of Pakistan.</obo:IAO_0000115>
        <oboInOwl:hasOBONamespace>GAZ</oboInOwl:hasOBONamespace>
        <oboInOwl:id>GAZ:00080187</oboInOwl:id>
        <rdfs:label>Dera Bugti Tehsil</rdfs:label>
    </owl:NamedIndividual>
    


    <!-- http://purl.obolibrary.org/obo/GAZ_00080188 -->

    <owl:NamedIndividual rdf:about="http://purl.obolibrary.org/obo/GAZ_00080188">
        <obo:RO_0001025 rdf:resource="http://purl.obolibrary.org/obo/GAZ_00018488"/>
        <obo:IAO_0000115>A Subdistrict of Gwadar District, Balochistan.</obo:IAO_0000115>
        <oboInOwl:hasOBONamespace>GAZ</oboInOwl:hasOBONamespace>
        <oboInOwl:id>GAZ:00080188</oboInOwl:id>
        <rdfs:label>Pasni Subdistrict</rdfs:label>
    </owl:NamedIndividual>
    


    <!-- http://purl.obolibrary.org/obo/GAZ_00080189 -->

    <owl:NamedIndividual rdf:about="http://purl.obolibrary.org/obo/GAZ_00080189">
        <obo:RO_0001025 rdf:resource="http://purl.obolibrary.org/obo/GAZ_00080188"/>
        <obo:IAO_0000115>A Tehsil in Gwadar District, Balochistan.</obo:IAO_0000115>
        <oboInOwl:hasOBONamespace>GAZ</oboInOwl:hasOBONamespace>
        <oboInOwl:id>GAZ:00080189</oboInOwl:id>
        <rdfs:label>Pasni Tehsil</rdfs:label>
    </owl:NamedIndividual>
    


    <!-- http://purl.obolibrary.org/obo/GAZ_00080190 -->

    <owl:NamedIndividual rdf:about="http://purl.obolibrary.org/obo/GAZ_00080190">
        <obo:RO_0001025 rdf:resource="http://purl.obolibrary.org/obo/GAZ_00018488"/>
        <obo:IAO_0000115>A Subdistrict of Gwadar District, Balochistan.</obo:IAO_0000115>
        <oboInOwl:hasOBONamespace>GAZ</oboInOwl:hasOBONamespace>
        <oboInOwl:id>GAZ:00080190</oboInOwl:id>
        <rdfs:label>Gwadar Subdistrict</rdfs:label>
    </owl:NamedIndividual>
    


    <!-- http://purl.obolibrary.org/obo/GAZ_00080191 -->

    <owl:NamedIndividual rdf:about="http://purl.obolibrary.org/obo/GAZ_00080191">
        <obo:RO_0001025 rdf:resource="http://purl.obolibrary.org/obo/GAZ_00080190"/>
        <obo:IAO_0000115>A Tehsil in Gwadar District, Balochistan, located along Arabian Sea in Gwadar District, Balochistan, Pakistan. It is located near the Iranian border.</obo:IAO_0000115>
        <oboInOwl:hasOBONamespace>GAZ</oboInOwl:hasOBONamespace>
        <oboInOwl:id>GAZ:00080191</oboInOwl:id>
        <rdfs:label>Jiwani Tehsil</rdfs:label>
    </owl:NamedIndividual>
    


    <!-- http://purl.obolibrary.org/obo/GAZ_00080192 -->

    <owl:NamedIndividual rdf:about="http://purl.obolibrary.org/obo/GAZ_00080192">
        <obo:RO_0001025 rdf:resource="http://purl.obolibrary.org/obo/GAZ_00080190"/>
        <obo:IAO_0000115>A Tehsil in Gwadar District, Balochistan.</obo:IAO_0000115>
        <oboInOwl:hasOBONamespace>GAZ</oboInOwl:hasOBONamespace>
        <oboInOwl:id>GAZ:00080192</oboInOwl:id>
        <rdfs:label>Gwadar Tehsil</rdfs:label>
    </owl:NamedIndividual>
    


    <!-- http://purl.obolibrary.org/obo/GAZ_00080193 -->

    <owl:NamedIndividual rdf:about="http://purl.obolibrary.org/obo/GAZ_00080193">
        <obo:RO_0001025 rdf:resource="http://purl.obolibrary.org/obo/GAZ_00080188"/>
        <obo:IAO_0000115>A Tehsil in Gwadar District, Balochistan.</obo:IAO_0000115>
        <oboInOwl:hasOBONamespace>GAZ</oboInOwl:hasOBONamespace>
        <oboInOwl:id>GAZ:00080193</oboInOwl:id>
        <rdfs:label>Ormara Tehsil</rdfs:label>
    </owl:NamedIndividual>
    


    <!-- http://purl.obolibrary.org/obo/GAZ_00080195 -->

    <owl:NamedIndividual rdf:about="http://purl.obolibrary.org/obo/GAZ_00080195">
        <obo:RO_0001025 rdf:resource="http://purl.obolibrary.org/obo/GAZ_00400002"/>
        <obo:IAO_0000115>One of the 4 Tehsils of Jafarabad District, Balochistan.</obo:IAO_0000115>
        <oboInOwl:hasOBONamespace>GAZ</oboInOwl:hasOBONamespace>
        <oboInOwl:id>GAZ:00080195</oboInOwl:id>
        <rdfs:label>Usta Mohammad Tehsil</rdfs:label>
    </owl:NamedIndividual>
    


    <!-- http://purl.obolibrary.org/obo/GAZ_00080196 -->

    <owl:NamedIndividual rdf:about="http://purl.obolibrary.org/obo/GAZ_00080196">
        <obo:RO_0001025 rdf:resource="http://purl.obolibrary.org/obo/GAZ_00400002"/>
        <obo:IAO_0000115>One of the 4 Tehsils of Jafarabad District, Balochistan.</obo:IAO_0000115>
        <oboInOwl:hasOBONamespace>GAZ</oboInOwl:hasOBONamespace>
        <oboInOwl:id>GAZ:00080196</oboInOwl:id>
        <rdfs:label>Jhat Pat Tehsil</rdfs:label>
    </owl:NamedIndividual>
    


    <!-- http://purl.obolibrary.org/obo/GAZ_00080197 -->

    <owl:NamedIndividual rdf:about="http://purl.obolibrary.org/obo/GAZ_00080197">
        <obo:RO_0001025 rdf:resource="http://purl.obolibrary.org/obo/GAZ_00400002"/>
        <obo:IAO_0000115>One of the 4 Tehsils of Jafarabad District, Balochistan.</obo:IAO_0000115>
        <oboInOwl:hasOBONamespace>GAZ</oboInOwl:hasOBONamespace>
        <oboInOwl:id>GAZ:00080197</oboInOwl:id>
        <rdfs:label>Suhbat Pur Tehsil</rdfs:label>
    </owl:NamedIndividual>
    


    <!-- http://purl.obolibrary.org/obo/GAZ_00080198 -->

    <owl:NamedIndividual rdf:about="http://purl.obolibrary.org/obo/GAZ_00080198">
        <obo:RO_0001025 rdf:resource="http://purl.obolibrary.org/obo/GAZ_00400002"/>
        <obo:IAO_0000115>One of the 4 Tehsils of Jafarabad District, Balochistan.</obo:IAO_0000115>
        <oboInOwl:hasOBONamespace>GAZ</oboInOwl:hasOBONamespace>
        <oboInOwl:id>GAZ:00080198</oboInOwl:id>
        <rdfs:label>Gandakha Tehsil</rdfs:label>
    </owl:NamedIndividual>
    


    <!-- http://purl.obolibrary.org/obo/GAZ_00080199 -->

    <owl:NamedIndividual rdf:about="http://purl.obolibrary.org/obo/GAZ_00080199">
        <obo:RO_0001025 rdf:resource="http://purl.obolibrary.org/obo/GAZ_00400022"/>
        <obo:IAO_0000115>A Subdistrict of the Jhal Magsi District, Balochistan.</obo:IAO_0000115>
        <oboInOwl:hasOBONamespace>GAZ</oboInOwl:hasOBONamespace>
        <oboInOwl:id>GAZ:00080199</oboInOwl:id>
        <rdfs:label>Gandawah Subdistrict</rdfs:label>
    </owl:NamedIndividual>
    


    <!-- http://purl.obolibrary.org/obo/GAZ_00080200 -->

    <owl:NamedIndividual rdf:about="http://purl.obolibrary.org/obo/GAZ_00080200">
        <obo:RO_0001025 rdf:resource="http://purl.obolibrary.org/obo/GAZ_00400022"/>
        <obo:IAO_0000115>A Subdistrict of the Jhal Magsi District, Balochistan.</obo:IAO_0000115>
        <oboInOwl:hasOBONamespace>GAZ</oboInOwl:hasOBONamespace>
        <oboInOwl:id>GAZ:00080200</oboInOwl:id>
        <rdfs:label>Jhal Magsi Subdistrict</rdfs:label>
    </owl:NamedIndividual>
    


    <!-- http://purl.obolibrary.org/obo/GAZ_00080201 -->

    <owl:NamedIndividual rdf:about="http://purl.obolibrary.org/obo/GAZ_00080201">
        <obo:RO_0001025 rdf:resource="http://purl.obolibrary.org/obo/GAZ_00400017"/>
        <obo:IAO_0000115>One of the 4 Tehsils of Kalat District, Balochistan.</obo:IAO_0000115>
        <oboInOwl:hasOBONamespace>GAZ</oboInOwl:hasOBONamespace>
        <oboInOwl:id>GAZ:00080201</oboInOwl:id>
        <rdfs:label>Gazg Johan Tehsil</rdfs:label>
    </owl:NamedIndividual>
    


    <!-- http://purl.obolibrary.org/obo/GAZ_00080202 -->

    <owl:NamedIndividual rdf:about="http://purl.obolibrary.org/obo/GAZ_00080202">
        <obo:RO_0001025 rdf:resource="http://purl.obolibrary.org/obo/GAZ_00400017"/>
        <obo:IAO_0000115>One of the 4 Tehsils of Kalat District, Balochistan.</obo:IAO_0000115>
        <oboInOwl:hasOBONamespace>GAZ</oboInOwl:hasOBONamespace>
        <oboInOwl:id>GAZ:00080202</oboInOwl:id>
        <rdfs:label>Kalat Tehsil</rdfs:label>
    </owl:NamedIndividual>
    


    <!-- http://purl.obolibrary.org/obo/GAZ_00080203 -->

    <owl:NamedIndividual rdf:about="http://purl.obolibrary.org/obo/GAZ_00080203">
        <obo:RO_0001025 rdf:resource="http://purl.obolibrary.org/obo/GAZ_00400017"/>
        <obo:IAO_0000115>One of the 4 Tehsils of Kalat District, Balochistan.</obo:IAO_0000115>
        <oboInOwl:hasOBONamespace>GAZ</oboInOwl:hasOBONamespace>
        <oboInOwl:id>GAZ:00080203</oboInOwl:id>
        <rdfs:label>Surab Tehsil</rdfs:label>
    </owl:NamedIndividual>
    


    <!-- http://purl.obolibrary.org/obo/GAZ_00080204 -->

    <owl:NamedIndividual rdf:about="http://purl.obolibrary.org/obo/GAZ_00080204">
        <obo:RO_0001025 rdf:resource="http://purl.obolibrary.org/obo/GAZ_00400017"/>
        <obo:IAO_0000115>One of the 4 Tehsils of Kalat District, Balochistan.</obo:IAO_0000115>
        <oboInOwl:hasOBONamespace>GAZ</oboInOwl:hasOBONamespace>
        <oboInOwl:id>GAZ:00080204</oboInOwl:id>
        <rdfs:label>Mangochar Tehsil</rdfs:label>
    </owl:NamedIndividual>
    


    <!-- http://purl.obolibrary.org/obo/GAZ_00080205 -->

    <owl:NamedIndividual rdf:about="http://purl.obolibrary.org/obo/GAZ_00080205">
        <obo:RO_0001025 rdf:resource="http://purl.obolibrary.org/obo/GAZ_00080214"/>
        <obo:IAO_0000115>A Tehsil of Kech District, Balochistan.</obo:IAO_0000115>
        <oboInOwl:hasOBONamespace>GAZ</oboInOwl:hasOBONamespace>
        <oboInOwl:id>GAZ:00080205</oboInOwl:id>
        <rdfs:label>Buleda Tehsil</rdfs:label>
    </owl:NamedIndividual>
    


    <!-- http://purl.obolibrary.org/obo/GAZ_00080206 -->

    <owl:NamedIndividual rdf:about="http://purl.obolibrary.org/obo/GAZ_00080206">
        <obo:RO_0001025 rdf:resource="http://purl.obolibrary.org/obo/GAZ_00080218"/>
        <obo:IAO_0000115>A Tehsil of Kech District, Balochistan.</obo:IAO_0000115>
        <oboInOwl:hasOBONamespace>GAZ</oboInOwl:hasOBONamespace>
        <oboInOwl:id>GAZ:00080206</oboInOwl:id>
        <rdfs:label>Mand Tehsil</rdfs:label>
    </owl:NamedIndividual>
    


    <!-- http://purl.obolibrary.org/obo/GAZ_00080207 -->

    <owl:NamedIndividual rdf:about="http://purl.obolibrary.org/obo/GAZ_00080207">
        <obo:RO_0001025 rdf:resource="http://purl.obolibrary.org/obo/GAZ_00400012"/>
        <obo:IAO_0000115>A Tehsil of Kech District, Balochistan.</obo:IAO_0000115>
        <oboInOwl:hasOBONamespace>GAZ</oboInOwl:hasOBONamespace>
        <oboInOwl:id>GAZ:00080207</oboInOwl:id>
        <rdfs:label>Zamoran Tehsil</rdfs:label>
    </owl:NamedIndividual>
    


    <!-- http://purl.obolibrary.org/obo/GAZ_00080208 -->

    <owl:NamedIndividual rdf:about="http://purl.obolibrary.org/obo/GAZ_00080208">
        <obo:RO_0001025 rdf:resource="http://purl.obolibrary.org/obo/GAZ_00080216"/>
        <obo:IAO_0000115>A Tehsil of Kech District, Balochistan.</obo:IAO_0000115>
        <oboInOwl:hasOBONamespace>GAZ</oboInOwl:hasOBONamespace>
        <oboInOwl:id>GAZ:00080208</oboInOwl:id>
        <rdfs:label>Dasht Tehsil</rdfs:label>
    </owl:NamedIndividual>
    


    <!-- http://purl.obolibrary.org/obo/GAZ_00080209 -->

    <owl:NamedIndividual rdf:about="http://purl.obolibrary.org/obo/GAZ_00080209">
        <obo:RO_0001025 rdf:resource="http://purl.obolibrary.org/obo/GAZ_00080218"/>
        <obo:IAO_0000115>A Tehsil of Kech District, Balochistan.</obo:IAO_0000115>
        <oboInOwl:hasOBONamespace>GAZ</oboInOwl:hasOBONamespace>
        <oboInOwl:id>GAZ:00080209</oboInOwl:id>
        <rdfs:label>Tump Tehsil</rdfs:label>
    </owl:NamedIndividual>
    


    <!-- http://purl.obolibrary.org/obo/GAZ_00080210 -->

    <owl:NamedIndividual rdf:about="http://purl.obolibrary.org/obo/GAZ_00080210">
        <obo:RO_0001025 rdf:resource="http://purl.obolibrary.org/obo/GAZ_00080213"/>
        <obo:IAO_0000115>A Tehsil of Kech District, Balochistan.</obo:IAO_0000115>
        <oboInOwl:hasOBONamespace>GAZ</oboInOwl:hasOBONamespace>
        <oboInOwl:id>GAZ:00080210</oboInOwl:id>
        <rdfs:label>Hoshab Tehsil</rdfs:label>
    </owl:NamedIndividual>
    


    <!-- http://purl.obolibrary.org/obo/GAZ_00080211 -->

    <owl:NamedIndividual rdf:about="http://purl.obolibrary.org/obo/GAZ_00080211">
        <obo:RO_0001025 rdf:resource="http://purl.obolibrary.org/obo/GAZ_00080213"/>
        <obo:IAO_0000115>A Tehsil of Kech District, Balochistan.</obo:IAO_0000115>
        <oboInOwl:hasOBONamespace>GAZ</oboInOwl:hasOBONamespace>
        <oboInOwl:id>GAZ:00080211</oboInOwl:id>
        <rdfs:label>Kech Tehsil</rdfs:label>
    </owl:NamedIndividual>
    


    <!-- http://purl.obolibrary.org/obo/GAZ_00080212 -->

    <owl:NamedIndividual rdf:about="http://purl.obolibrary.org/obo/GAZ_00080212">
        <obo:RO_0001025 rdf:resource="http://purl.obolibrary.org/obo/GAZ_00080216"/>
        <obo:IAO_0000115>A Tehsil of Kech District, Balochistan.</obo:IAO_0000115>
        <oboInOwl:hasOBONamespace>GAZ</oboInOwl:hasOBONamespace>
        <oboInOwl:id>GAZ:00080212</oboInOwl:id>
        <rdfs:label>Balingor Tehsil</rdfs:label>
    </owl:NamedIndividual>
    


    <!-- http://purl.obolibrary.org/obo/GAZ_00080213 -->

    <owl:NamedIndividual rdf:about="http://purl.obolibrary.org/obo/GAZ_00080213">
        <obo:RO_0001025 rdf:resource="http://purl.obolibrary.org/obo/GAZ_00400012"/>
        <obo:IAO_0000115>A Subdistrict of Kech District, Balochistan.</obo:IAO_0000115>
        <oboInOwl:hasOBONamespace>GAZ</oboInOwl:hasOBONamespace>
        <oboInOwl:id>GAZ:00080213</oboInOwl:id>
        <rdfs:label>Turbat Subdistrict</rdfs:label>
    </owl:NamedIndividual>
    


    <!-- http://purl.obolibrary.org/obo/GAZ_00080214 -->

    <owl:NamedIndividual rdf:about="http://purl.obolibrary.org/obo/GAZ_00080214">
        <obo:RO_0001025 rdf:resource="http://purl.obolibrary.org/obo/GAZ_00400012"/>
        <obo:IAO_0000115>A Subdistrict of Kech District, Balochistan.</obo:IAO_0000115>
        <oboInOwl:hasOBONamespace>GAZ</oboInOwl:hasOBONamespace>
        <oboInOwl:id>GAZ:00080214</oboInOwl:id>
        <rdfs:label>Buleda Subdistrict</rdfs:label>
    </owl:NamedIndividual>
    


    <!-- http://purl.obolibrary.org/obo/GAZ_00080215 -->

    <owl:NamedIndividual rdf:about="http://purl.obolibrary.org/obo/GAZ_00080215">
        <obo:RO_0001025 rdf:resource="http://purl.obolibrary.org/obo/GAZ_00080214"/>
        <obo:IAO_0000115>A Tehsil of Kech District, Balochistan.</obo:IAO_0000115>
        <oboInOwl:hasOBONamespace>GAZ</oboInOwl:hasOBONamespace>
        <oboInOwl:id>GAZ:00080215</oboInOwl:id>
        <rdfs:label>Niwano Tehsil</rdfs:label>
    </owl:NamedIndividual>
    


    <!-- http://purl.obolibrary.org/obo/GAZ_00080216 -->

    <owl:NamedIndividual rdf:about="http://purl.obolibrary.org/obo/GAZ_00080216">
        <obo:RO_0001025 rdf:resource="http://purl.obolibrary.org/obo/GAZ_00400012"/>
        <obo:IAO_0000115>A Subdistrict of Kech District, Balochistan.</obo:IAO_0000115>
        <oboInOwl:hasOBONamespace>GAZ</oboInOwl:hasOBONamespace>
        <oboInOwl:id>GAZ:00080216</oboInOwl:id>
        <rdfs:label>Dasht Subdistrict</rdfs:label>
    </owl:NamedIndividual>
    


    <!-- http://purl.obolibrary.org/obo/GAZ_00080217 -->

    <owl:NamedIndividual rdf:about="http://purl.obolibrary.org/obo/GAZ_00080217">
        <obo:RO_0001025 rdf:resource="http://purl.obolibrary.org/obo/GAZ_00400025"/>
        <obo:IAO_0000115>A Tehsil of Kharan District, Balochistan.</obo:IAO_0000115>
        <oboInOwl:hasOBONamespace>GAZ</oboInOwl:hasOBONamespace>
        <oboInOwl:id>GAZ:00080217</oboInOwl:id>
        <rdfs:label>Mashkel Tehsil</rdfs:label>
    </owl:NamedIndividual>
    


    <!-- http://purl.obolibrary.org/obo/GAZ_00080218 -->

    <owl:NamedIndividual rdf:about="http://purl.obolibrary.org/obo/GAZ_00080218">
        <obo:RO_0001025 rdf:resource="http://purl.obolibrary.org/obo/GAZ_00400012"/>
        <obo:IAO_0000115>A Subdistrict of Kech District, Balochistan.</obo:IAO_0000115>
        <oboInOwl:hasOBONamespace>GAZ</oboInOwl:hasOBONamespace>
        <oboInOwl:id>GAZ:00080218</oboInOwl:id>
        <rdfs:label>Tump Subdistrict</rdfs:label>
    </owl:NamedIndividual>
    


    <!-- http://purl.obolibrary.org/obo/GAZ_00080219 -->

    <owl:NamedIndividual rdf:about="http://purl.obolibrary.org/obo/GAZ_00080219">
        <obo:RO_0001025 rdf:resource="http://purl.obolibrary.org/obo/GAZ_00400025"/>
        <obo:IAO_0000115>A Tehsil of Kharan District, Balochistan.</obo:IAO_0000115>
        <oboInOwl:hasOBONamespace>GAZ</oboInOwl:hasOBONamespace>
        <oboInOwl:id>GAZ:00080219</oboInOwl:id>
        <rdfs:label>Besima Tehsil</rdfs:label>
    </owl:NamedIndividual>
    


    <!-- http://purl.obolibrary.org/obo/GAZ_00080220 -->

    <owl:NamedIndividual rdf:about="http://purl.obolibrary.org/obo/GAZ_00080220">
        <obo:RO_0001025 rdf:resource="http://purl.obolibrary.org/obo/GAZ_00400025"/>
        <obo:IAO_0000115>A Tehsil of Kharan District, Balochistan.</obo:IAO_0000115>
        <oboInOwl:hasOBONamespace>GAZ</oboInOwl:hasOBONamespace>
        <oboInOwl:id>GAZ:00080220</oboInOwl:id>
        <rdfs:label>Nag Tehsil</rdfs:label>
    </owl:NamedIndividual>
    


    <!-- http://purl.obolibrary.org/obo/GAZ_00080221 -->

    <owl:NamedIndividual rdf:about="http://purl.obolibrary.org/obo/GAZ_00080221">
        <obo:RO_0001025 rdf:resource="http://purl.obolibrary.org/obo/GAZ_00400025"/>
        <obo:IAO_0000115>A Tehsil of Kharan District, Balochistan.</obo:IAO_0000115>
        <oboInOwl:hasOBONamespace>GAZ</oboInOwl:hasOBONamespace>
        <oboInOwl:id>GAZ:00080221</oboInOwl:id>
        <rdfs:label>Kharan Tehsil</rdfs:label>
    </owl:NamedIndividual>
    


    <!-- http://purl.obolibrary.org/obo/GAZ_00080222 -->

    <owl:NamedIndividual rdf:about="http://purl.obolibrary.org/obo/GAZ_00080222">
        <obo:RO_0001025 rdf:resource="http://purl.obolibrary.org/obo/GAZ_00400025"/>
        <obo:IAO_0000115>A Tehsil of Kharan District, Balochistan.</obo:IAO_0000115>
        <oboInOwl:hasOBONamespace>GAZ</oboInOwl:hasOBONamespace>
        <oboInOwl:id>GAZ:00080222</oboInOwl:id>
        <rdfs:label>Wasuk Tehsil</rdfs:label>
    </owl:NamedIndividual>
    


    <!-- http://purl.obolibrary.org/obo/GAZ_00080223 -->

    <owl:NamedIndividual rdf:about="http://purl.obolibrary.org/obo/GAZ_00080223">
        <obo:RO_0001025 rdf:resource="http://purl.obolibrary.org/obo/GAZ_00400023"/>
        <obo:IAO_0000115>A Tehsil in Kohlu District, Balochistan.</obo:IAO_0000115>
        <oboInOwl:hasOBONamespace>GAZ</oboInOwl:hasOBONamespace>
        <oboInOwl:id>GAZ:00080223</oboInOwl:id>
        <rdfs:label>Maiwand Tehsil</rdfs:label>
    </owl:NamedIndividual>
    


    <!-- http://purl.obolibrary.org/obo/GAZ_00080224 -->

    <owl:NamedIndividual rdf:about="http://purl.obolibrary.org/obo/GAZ_00080224">
        <obo:RO_0001025 rdf:resource="http://purl.obolibrary.org/obo/GAZ_00400023"/>
        <obo:IAO_0000115>A Tehsil in Kohlu District, Balochistan.</obo:IAO_0000115>
        <oboInOwl:hasOBONamespace>GAZ</oboInOwl:hasOBONamespace>
        <oboInOwl:id>GAZ:00080224</oboInOwl:id>
        <rdfs:label>Kohlu Tehsil</rdfs:label>
    </owl:NamedIndividual>
    


    <!-- http://purl.obolibrary.org/obo/GAZ_00080225 -->

    <owl:NamedIndividual rdf:about="http://purl.obolibrary.org/obo/GAZ_00080225">
        <obo:RO_0001025 rdf:resource="http://purl.obolibrary.org/obo/GAZ_00400023"/>
        <obo:IAO_0000115>A Tehsil in Kohlu District, Balochistan.</obo:IAO_0000115>
        <oboInOwl:hasOBONamespace>GAZ</oboInOwl:hasOBONamespace>
        <oboInOwl:id>GAZ:00080225</oboInOwl:id>
        <rdfs:label>Kahan Tehsil</rdfs:label>
    </owl:NamedIndividual>
    


    <!-- http://purl.obolibrary.org/obo/GAZ_00080226 -->

    <owl:NamedIndividual rdf:about="http://purl.obolibrary.org/obo/GAZ_00080226">
        <obo:RO_0001025 rdf:resource="http://purl.obolibrary.org/obo/GAZ_00400018"/>
        <obo:IAO_0000115>A Tehsil in Khuzdar District, Balochistan.</obo:IAO_0000115>
        <oboInOwl:hasOBONamespace>GAZ</oboInOwl:hasOBONamespace>
        <oboInOwl:id>GAZ:00080226</oboInOwl:id>
        <rdfs:label>Karkh Tehsil</rdfs:label>
    </owl:NamedIndividual>
    


    <!-- http://purl.obolibrary.org/obo/GAZ_00080227 -->

    <owl:NamedIndividual rdf:about="http://purl.obolibrary.org/obo/GAZ_00080227">
        <obo:RO_0001025 rdf:resource="http://purl.obolibrary.org/obo/GAZ_00400018"/>
        <obo:IAO_0000115>A Tehsil in Khuzdar District, Balochistan.</obo:IAO_0000115>
        <oboInOwl:hasOBONamespace>GAZ</oboInOwl:hasOBONamespace>
        <oboInOwl:id>GAZ:00080227</oboInOwl:id>
        <rdfs:label>Wadh Tehsil</rdfs:label>
    </owl:NamedIndividual>
    


    <!-- http://purl.obolibrary.org/obo/GAZ_00080228 -->

    <owl:NamedIndividual rdf:about="http://purl.obolibrary.org/obo/GAZ_00080228">
        <obo:RO_0001025 rdf:resource="http://purl.obolibrary.org/obo/GAZ_00400018"/>
        <obo:IAO_0000115>A Tehsil in Khuzdar District, Balochistan.</obo:IAO_0000115>
        <oboInOwl:hasOBONamespace>GAZ</oboInOwl:hasOBONamespace>
        <oboInOwl:id>GAZ:00080228</oboInOwl:id>
        <rdfs:label>Zehri Tehsil</rdfs:label>
    </owl:NamedIndividual>
    


    <!-- http://purl.obolibrary.org/obo/GAZ_00080229 -->

    <owl:NamedIndividual rdf:about="http://purl.obolibrary.org/obo/GAZ_00080229">
        <obo:RO_0001025 rdf:resource="http://purl.obolibrary.org/obo/GAZ_00400018"/>
        <obo:IAO_0000115>A Tehsil in Khuzdar District, Balochistan.</obo:IAO_0000115>
        <oboInOwl:hasOBONamespace>GAZ</oboInOwl:hasOBONamespace>
        <oboInOwl:id>GAZ:00080229</oboInOwl:id>
        <rdfs:label>Naal Tehsil</rdfs:label>
    </owl:NamedIndividual>
    


    <!-- http://purl.obolibrary.org/obo/GAZ_00080230 -->

    <owl:NamedIndividual rdf:about="http://purl.obolibrary.org/obo/GAZ_00080230">
        <obo:RO_0001025 rdf:resource="http://purl.obolibrary.org/obo/GAZ_00400018"/>
        <obo:IAO_0000115>A Tehsil in Khuzdar District, Balochistan.</obo:IAO_0000115>
        <oboInOwl:hasOBONamespace>GAZ</oboInOwl:hasOBONamespace>
        <oboInOwl:id>GAZ:00080230</oboInOwl:id>
        <rdfs:label>Khuzdar Tehsil</rdfs:label>
    </owl:NamedIndividual>
    


    <!-- http://purl.obolibrary.org/obo/GAZ_00080231 -->

    <owl:NamedIndividual rdf:about="http://purl.obolibrary.org/obo/GAZ_00080231">
        <obo:RO_0001025 rdf:resource="http://purl.obolibrary.org/obo/GAZ_00400026"/>
        <obo:IAO_0000115>A Tehsil of Qilla Abdullah District, Balochistan.</obo:IAO_0000115>
        <oboInOwl:hasOBONamespace>GAZ</oboInOwl:hasOBONamespace>
        <oboInOwl:id>GAZ:00080231</oboInOwl:id>
        <rdfs:label>Chaman Tehsil</rdfs:label>
    </owl:NamedIndividual>
    


    <!-- http://purl.obolibrary.org/obo/GAZ_00080232 -->

    <owl:NamedIndividual rdf:about="http://purl.obolibrary.org/obo/GAZ_00080232">
        <obo:RO_0001025 rdf:resource="http://purl.obolibrary.org/obo/GAZ_00400026"/>
        <obo:IAO_0000115>A Tehsil of Qilla Abdullah District, Balochistan.</obo:IAO_0000115>
        <oboInOwl:hasOBONamespace>GAZ</oboInOwl:hasOBONamespace>
        <oboInOwl:id>GAZ:00080232</oboInOwl:id>
        <rdfs:label>Dobandi Tehsil</rdfs:label>
    </owl:NamedIndividual>
    


    <!-- http://purl.obolibrary.org/obo/GAZ_00080233 -->

    <owl:NamedIndividual rdf:about="http://purl.obolibrary.org/obo/GAZ_00080233">
        <obo:RO_0001025 rdf:resource="http://purl.obolibrary.org/obo/GAZ_00400026"/>
        <obo:IAO_0000115>A Tehsil of Qilla Abdullah District, Balochistan.</obo:IAO_0000115>
        <oboInOwl:hasOBONamespace>GAZ</oboInOwl:hasOBONamespace>
        <oboInOwl:id>GAZ:00080233</oboInOwl:id>
        <rdfs:label>Gulistan Tehsil</rdfs:label>
    </owl:NamedIndividual>
    


    <!-- http://purl.obolibrary.org/obo/GAZ_00080234 -->

    <owl:NamedIndividual rdf:about="http://purl.obolibrary.org/obo/GAZ_00080234">
        <obo:RO_0001025 rdf:resource="http://purl.obolibrary.org/obo/GAZ_00400026"/>
        <obo:IAO_0000115>A Tehsil of Qilla Abdullah District, Balochistan.</obo:IAO_0000115>
        <oboInOwl:hasOBONamespace>GAZ</oboInOwl:hasOBONamespace>
        <oboInOwl:id>GAZ:00080234</oboInOwl:id>
        <rdfs:label>Qilla Abdullah Tehsil</rdfs:label>
    </owl:NamedIndividual>
    


    <!-- http://purl.obolibrary.org/obo/GAZ_00080235 -->

    <owl:NamedIndividual rdf:about="http://purl.obolibrary.org/obo/GAZ_00080235">
        <obo:RO_0001025 rdf:resource="http://purl.obolibrary.org/obo/GAZ_00400024"/>
        <obo:IAO_0000115>A Subdistrict of Qilla Saifullah District, Balochistan.</obo:IAO_0000115>
        <oboInOwl:hasOBONamespace>GAZ</oboInOwl:hasOBONamespace>
        <oboInOwl:id>GAZ:00080235</oboInOwl:id>
        <rdfs:label>Muslim Bagh Subdistrict</rdfs:label>
    </owl:NamedIndividual>
    


    <!-- http://purl.obolibrary.org/obo/GAZ_00080236 -->

    <owl:NamedIndividual rdf:about="http://purl.obolibrary.org/obo/GAZ_00080236">
        <obo:RO_0001025 rdf:resource="http://purl.obolibrary.org/obo/GAZ_00080235"/>
        <obo:IAO_0000115>A Tehsil of Qilla Saifullah District, Balochistan.</obo:IAO_0000115>
        <oboInOwl:hasOBONamespace>GAZ</oboInOwl:hasOBONamespace>
        <oboInOwl:id>GAZ:00080236</oboInOwl:id>
        <rdfs:label>Muslim Bagh Tehsil</rdfs:label>
    </owl:NamedIndividual>
    


    <!-- http://purl.obolibrary.org/obo/GAZ_00080237 -->

    <owl:NamedIndividual rdf:about="http://purl.obolibrary.org/obo/GAZ_00080237">
        <obo:RO_0001025 rdf:resource="http://purl.obolibrary.org/obo/GAZ_00400024"/>
        <obo:IAO_0000115>A Subdistrict of Qilla Saifullah District, Balochistan.</obo:IAO_0000115>
        <oboInOwl:hasOBONamespace>GAZ</oboInOwl:hasOBONamespace>
        <oboInOwl:id>GAZ:00080237</oboInOwl:id>
        <rdfs:label>Qilla Saifullah Subdistrict</rdfs:label>
    </owl:NamedIndividual>
    


    <!-- http://purl.obolibrary.org/obo/GAZ_00080238 -->

    <owl:NamedIndividual rdf:about="http://purl.obolibrary.org/obo/GAZ_00080238">
        <obo:RO_0001025 rdf:resource="http://purl.obolibrary.org/obo/GAZ_00080237"/>
        <obo:IAO_0000115>A Tehsil of Qilla Saifullah District, Balochistan.</obo:IAO_0000115>
        <oboInOwl:hasOBONamespace>GAZ</oboInOwl:hasOBONamespace>
        <oboInOwl:id>GAZ:00080238</oboInOwl:id>
        <rdfs:label>Qilla Saifullah Tehsil</rdfs:label>
    </owl:NamedIndividual>
    


    <!-- http://purl.obolibrary.org/obo/GAZ_00080239 -->

    <owl:NamedIndividual rdf:about="http://purl.obolibrary.org/obo/GAZ_00080239">
        <obo:RO_0001025 rdf:resource="http://purl.obolibrary.org/obo/GAZ_00080235"/>
        <obo:IAO_0000115>A Sub-Tehsil of Qilla Saifullah District, Balochistan.</obo:IAO_0000115>
        <oboInOwl:hasOBONamespace>GAZ</oboInOwl:hasOBONamespace>
        <oboInOwl:id>GAZ:00080239</oboInOwl:id>
        <rdfs:label>Loiband Sub-Tehsil</rdfs:label>
    </owl:NamedIndividual>
    


    <!-- http://purl.obolibrary.org/obo/GAZ_00080240 -->

    <owl:NamedIndividual rdf:about="http://purl.obolibrary.org/obo/GAZ_00080240">
        <obo:RO_0001025 rdf:resource="http://purl.obolibrary.org/obo/GAZ_00080237"/>
        <obo:IAO_0000115>A Sub-Tehsil of Qilla Saifullah District, Balochistan.</obo:IAO_0000115>
        <oboInOwl:hasOBONamespace>GAZ</oboInOwl:hasOBONamespace>
        <oboInOwl:id>GAZ:00080240</oboInOwl:id>
        <rdfs:label>Badinai Sub-Tehsil</rdfs:label>
    </owl:NamedIndividual>
    


    <!-- http://purl.obolibrary.org/obo/GAZ_00080241 -->

    <owl:NamedIndividual rdf:about="http://purl.obolibrary.org/obo/GAZ_00080241">
        <obo:RO_0001025 rdf:resource="http://purl.obolibrary.org/obo/GAZ_00400020"/>
        <obo:IAO_0000115>A Tehsil of Lasbela District, Balochistan.</obo:IAO_0000115>
        <oboInOwl:hasOBONamespace>GAZ</oboInOwl:hasOBONamespace>
        <oboInOwl:id>GAZ:00080241</oboInOwl:id>
        <rdfs:label>Hub Tehsil</rdfs:label>
    </owl:NamedIndividual>
    


    <!-- http://purl.obolibrary.org/obo/GAZ_00080242 -->

    <owl:NamedIndividual rdf:about="http://purl.obolibrary.org/obo/GAZ_00080242">
        <obo:RO_0001025 rdf:resource="http://purl.obolibrary.org/obo/GAZ_00400020"/>
        <obo:IAO_0000115>A Tehsil of Lasbela District, Balochistan.</obo:IAO_0000115>
        <oboInOwl:hasOBONamespace>GAZ</oboInOwl:hasOBONamespace>
        <oboInOwl:id>GAZ:00080242</oboInOwl:id>
        <rdfs:label>Uthal Tehsil</rdfs:label>
    </owl:NamedIndividual>
    


    <!-- http://purl.obolibrary.org/obo/GAZ_00080243 -->

    <owl:NamedIndividual rdf:about="http://purl.obolibrary.org/obo/GAZ_00080243">
        <obo:RO_0001025 rdf:resource="http://purl.obolibrary.org/obo/GAZ_00400020"/>
        <obo:IAO_0000115>A Tehsil of Lasbela District, Balochistan.</obo:IAO_0000115>
        <oboInOwl:hasOBONamespace>GAZ</oboInOwl:hasOBONamespace>
        <oboInOwl:id>GAZ:00080243</oboInOwl:id>
        <rdfs:label>Dureji Tehsil</rdfs:label>
    </owl:NamedIndividual>
    


    <!-- http://purl.obolibrary.org/obo/GAZ_00080244 -->

    <owl:NamedIndividual rdf:about="http://purl.obolibrary.org/obo/GAZ_00080244">
        <obo:RO_0001025 rdf:resource="http://purl.obolibrary.org/obo/GAZ_00400020"/>
        <obo:IAO_0000115>A Tehsil of Lasbela District, Balochistan.</obo:IAO_0000115>
        <oboInOwl:hasOBONamespace>GAZ</oboInOwl:hasOBONamespace>
        <oboInOwl:id>GAZ:00080244</oboInOwl:id>
        <rdfs:label>Bela Tehsil</rdfs:label>
    </owl:NamedIndividual>
    


    <!-- http://purl.obolibrary.org/obo/GAZ_00080245 -->

    <owl:NamedIndividual rdf:about="http://purl.obolibrary.org/obo/GAZ_00080245">
        <obo:RO_0001025 rdf:resource="http://purl.obolibrary.org/obo/GAZ_00400020"/>
        <obo:IAO_0000115>A Tehsil of Lasbela District, Balochistan.</obo:IAO_0000115>
        <oboInOwl:hasOBONamespace>GAZ</oboInOwl:hasOBONamespace>
        <oboInOwl:id>GAZ:00080245</oboInOwl:id>
        <rdfs:label>Sonmiani Tehsil</rdfs:label>
    </owl:NamedIndividual>
    


    <!-- http://purl.obolibrary.org/obo/GAZ_00080246 -->

    <owl:NamedIndividual rdf:about="http://purl.obolibrary.org/obo/GAZ_00080246">
        <obo:RO_0001025 rdf:resource="http://purl.obolibrary.org/obo/GAZ_00400020"/>
        <obo:IAO_0000115>A Tehsil of Lasbela District, Balochistan.</obo:IAO_0000115>
        <oboInOwl:hasOBONamespace>GAZ</oboInOwl:hasOBONamespace>
        <oboInOwl:id>GAZ:00080246</oboInOwl:id>
        <rdfs:label>Liari Tehsil</rdfs:label>
    </owl:NamedIndividual>
    


    <!-- http://purl.obolibrary.org/obo/GAZ_00080247 -->

    <owl:NamedIndividual rdf:about="http://purl.obolibrary.org/obo/GAZ_00080247">
        <obo:RO_0001025 rdf:resource="http://purl.obolibrary.org/obo/GAZ_00400020"/>
        <obo:IAO_0000115>A Tehsil of Lasbela District, Balochistan.</obo:IAO_0000115>
        <oboInOwl:hasOBONamespace>GAZ</oboInOwl:hasOBONamespace>
        <oboInOwl:id>GAZ:00080247</oboInOwl:id>
        <rdfs:label>Gadani Tehsil</rdfs:label>
    </owl:NamedIndividual>
    


    <!-- http://purl.obolibrary.org/obo/GAZ_00080248 -->

    <owl:NamedIndividual rdf:about="http://purl.obolibrary.org/obo/GAZ_00080248">
        <obo:RO_0001025 rdf:resource="http://purl.obolibrary.org/obo/GAZ_00400020"/>
        <obo:IAO_0000115>A Tehsil of Lasbela District, Balochistan.</obo:IAO_0000115>
        <oboInOwl:hasOBONamespace>GAZ</oboInOwl:hasOBONamespace>
        <oboInOwl:id>GAZ:00080248</oboInOwl:id>
        <rdfs:label>Lakhra Tehsil</rdfs:label>
    </owl:NamedIndividual>
    


    <!-- http://purl.obolibrary.org/obo/GAZ_00080249 -->

    <owl:NamedIndividual rdf:about="http://purl.obolibrary.org/obo/GAZ_00080249">
        <obo:RO_0001025 rdf:resource="http://purl.obolibrary.org/obo/GAZ_00400020"/>
        <obo:IAO_0000115>A Tehsil of Lasbela District, Balochistan.</obo:IAO_0000115>
        <oboInOwl:hasOBONamespace>GAZ</oboInOwl:hasOBONamespace>
        <oboInOwl:id>GAZ:00080249</oboInOwl:id>
        <rdfs:label>Kanraj Tehsil</rdfs:label>
    </owl:NamedIndividual>
    


    <!-- http://purl.obolibrary.org/obo/GAZ_00080250 -->

    <owl:NamedIndividual rdf:about="http://purl.obolibrary.org/obo/GAZ_00080250">
        <obo:RO_0001025 rdf:resource="http://purl.obolibrary.org/obo/GAZ_00400016"/>
        <obo:IAO_0000115>A Subdistrict of Loralai District, Balochistan.</obo:IAO_0000115>
        <oboInOwl:hasOBONamespace>GAZ</oboInOwl:hasOBONamespace>
        <oboInOwl:id>GAZ:00080250</oboInOwl:id>
        <rdfs:label>Bori Subdistrict</rdfs:label>
    </owl:NamedIndividual>
    


    <!-- http://purl.obolibrary.org/obo/GAZ_00080251 -->

    <owl:NamedIndividual rdf:about="http://purl.obolibrary.org/obo/GAZ_00080251">
        <obo:RO_0001025 rdf:resource="http://purl.obolibrary.org/obo/GAZ_00400016"/>
        <obo:IAO_0000115>A Subdistrict of Loralai District, Balochistan.</obo:IAO_0000115>
        <oboInOwl:hasOBONamespace>GAZ</oboInOwl:hasOBONamespace>
        <oboInOwl:id>GAZ:00080251</oboInOwl:id>
        <rdfs:label>Duki Subdistrict</rdfs:label>
    </owl:NamedIndividual>
    


    <!-- http://purl.obolibrary.org/obo/GAZ_00080252 -->

    <owl:NamedIndividual rdf:about="http://purl.obolibrary.org/obo/GAZ_00080252">
        <obo:RO_0001025 rdf:resource="http://purl.obolibrary.org/obo/GAZ_00080251"/>
        <obo:IAO_0000115>A Tehsil of Loralai District, Balochistan.</obo:IAO_0000115>
        <oboInOwl:hasOBONamespace>GAZ</oboInOwl:hasOBONamespace>
        <oboInOwl:id>GAZ:00080252</oboInOwl:id>
        <rdfs:label>Duki Tehsil</rdfs:label>
    </owl:NamedIndividual>
    


    <!-- http://purl.obolibrary.org/obo/GAZ_00080253 -->

    <owl:NamedIndividual rdf:about="http://purl.obolibrary.org/obo/GAZ_00080253">
        <obo:RO_0001025 rdf:resource="http://purl.obolibrary.org/obo/GAZ_00080250"/>
        <obo:IAO_0000115>A Tehsil of Loralai District, Balochistan.</obo:IAO_0000115>
        <oboInOwl:hasOBONamespace>GAZ</oboInOwl:hasOBONamespace>
        <oboInOwl:id>GAZ:00080253</oboInOwl:id>
        <rdfs:label>Bori Tehsil</rdfs:label>
    </owl:NamedIndividual>
    


    <!-- http://purl.obolibrary.org/obo/GAZ_00080254 -->

    <owl:NamedIndividual rdf:about="http://purl.obolibrary.org/obo/GAZ_00080254">
        <obo:RO_0001025 rdf:resource="http://purl.obolibrary.org/obo/GAZ_00080251"/>
        <obo:IAO_0000115>A Sub-Tehsil of Loralai District, Balochistan.</obo:IAO_0000115>
        <oboInOwl:hasOBONamespace>GAZ</oboInOwl:hasOBONamespace>
        <oboInOwl:id>GAZ:00080254</oboInOwl:id>
        <rdfs:label>Sinjavi Sub-Tehsil</rdfs:label>
    </owl:NamedIndividual>
    


    <!-- http://purl.obolibrary.org/obo/GAZ_00080255 -->

    <owl:NamedIndividual rdf:about="http://purl.obolibrary.org/obo/GAZ_00080255">
        <obo:RO_0001025 rdf:resource="http://purl.obolibrary.org/obo/GAZ_00080250"/>
        <obo:IAO_0000115>A Sub-Tehsil of Loralai District, Balochistan.</obo:IAO_0000115>
        <oboInOwl:hasOBONamespace>GAZ</oboInOwl:hasOBONamespace>
        <oboInOwl:id>GAZ:00080255</oboInOwl:id>
        <rdfs:label>Makhter Sub-Tehsil</rdfs:label>
    </owl:NamedIndividual>
    


    <!-- http://purl.obolibrary.org/obo/GAZ_00080256 -->

    <owl:NamedIndividual rdf:about="http://purl.obolibrary.org/obo/GAZ_00080256">
        <obo:RO_0001025 rdf:resource="http://purl.obolibrary.org/obo/GAZ_00400015"/>
        <obo:IAO_0000115>A Tehsil of Mastung District, Balochistan.</obo:IAO_0000115>
        <oboInOwl:hasOBONamespace>GAZ</oboInOwl:hasOBONamespace>
        <oboInOwl:id>GAZ:00080256</oboInOwl:id>
        <rdfs:label>Dasht Tehsil</rdfs:label>
    </owl:NamedIndividual>
    


    <!-- http://purl.obolibrary.org/obo/GAZ_00080257 -->

    <owl:NamedIndividual rdf:about="http://purl.obolibrary.org/obo/GAZ_00080257">
        <obo:RO_0001025 rdf:resource="http://purl.obolibrary.org/obo/GAZ_00400015"/>
        <obo:IAO_0000115>A Tehsil of Mastung District, Balochistan.</obo:IAO_0000115>
        <oboInOwl:hasOBONamespace>GAZ</oboInOwl:hasOBONamespace>
        <oboInOwl:id>GAZ:00080257</oboInOwl:id>
        <rdfs:label>Kardigap Tehsil</rdfs:label>
    </owl:NamedIndividual>
    


    <!-- http://purl.obolibrary.org/obo/GAZ_00080258 -->

    <owl:NamedIndividual rdf:about="http://purl.obolibrary.org/obo/GAZ_00080258">
        <obo:RO_0001025 rdf:resource="http://purl.obolibrary.org/obo/GAZ_00400015"/>
        <obo:IAO_0000115>A Tehsil of Mastung District, Balochistan.</obo:IAO_0000115>
        <oboInOwl:hasOBONamespace>GAZ</oboInOwl:hasOBONamespace>
        <oboInOwl:id>GAZ:00080258</oboInOwl:id>
        <rdfs:label>Mastung Tehsil</rdfs:label>
    </owl:NamedIndividual>
    


    <!-- http://purl.obolibrary.org/obo/GAZ_00080259 -->

    <owl:NamedIndividual rdf:about="http://purl.obolibrary.org/obo/GAZ_00080259">
        <obo:RO_0001025 rdf:resource="http://purl.obolibrary.org/obo/GAZ_00400019"/>
        <obo:IAO_0000115>A Tehsil of Masakhel District, Balochistan.</obo:IAO_0000115>
        <oboInOwl:hasOBONamespace>GAZ</oboInOwl:hasOBONamespace>
        <oboInOwl:id>GAZ:00080259</oboInOwl:id>
        <rdfs:label>Musakhel Tehsil</rdfs:label>
    </owl:NamedIndividual>
    


    <!-- http://purl.obolibrary.org/obo/GAZ_00080260 -->

    <owl:NamedIndividual rdf:about="http://purl.obolibrary.org/obo/GAZ_00080260">
        <obo:RO_0001025 rdf:resource="http://purl.obolibrary.org/obo/GAZ_00400019"/>
        <obo:IAO_0000115>A Sub-Tehsil of Masakhel District, Balochistan.</obo:IAO_0000115>
        <oboInOwl:hasOBONamespace>GAZ</oboInOwl:hasOBONamespace>
        <oboInOwl:id>GAZ:00080260</oboInOwl:id>
        <rdfs:label>Kingri Sub-Tehsil</rdfs:label>
    </owl:NamedIndividual>
    


    <!-- http://purl.obolibrary.org/obo/GAZ_00080261 -->

    <owl:NamedIndividual rdf:about="http://purl.obolibrary.org/obo/GAZ_00080261">
        <obo:RO_0001025 rdf:resource="http://purl.obolibrary.org/obo/GAZ_00400013"/>
        <obo:IAO_0000115>A Tehsil of Nasirabad District, Balochistan.</obo:IAO_0000115>
        <oboInOwl:hasOBONamespace>GAZ</oboInOwl:hasOBONamespace>
        <oboInOwl:id>GAZ:00080261</oboInOwl:id>
        <rdfs:label>Tamboo Tehsil</rdfs:label>
    </owl:NamedIndividual>
    


    <!-- http://purl.obolibrary.org/obo/GAZ_00080262 -->

    <owl:NamedIndividual rdf:about="http://purl.obolibrary.org/obo/GAZ_00080262">
        <obo:RO_0001025 rdf:resource="http://purl.obolibrary.org/obo/GAZ_00400013"/>
        <obo:IAO_0000115>A Subdistrict of Nasirabad District, Balochistan.</obo:IAO_0000115>
        <oboInOwl:hasOBONamespace>GAZ</oboInOwl:hasOBONamespace>
        <oboInOwl:id>GAZ:00080262</oboInOwl:id>
        <rdfs:label>Murad Jamali Subdistrict</rdfs:label>
    </owl:NamedIndividual>
    


    <!-- http://purl.obolibrary.org/obo/GAZ_00080263 -->

    <owl:NamedIndividual rdf:about="http://purl.obolibrary.org/obo/GAZ_00080263">
        <obo:RO_0001025 rdf:resource="http://purl.obolibrary.org/obo/GAZ_00400013"/>
        <obo:IAO_0000115>A Subdistrict of Nasirabad District, Balochistan.</obo:IAO_0000115>
        <oboInOwl:hasOBONamespace>GAZ</oboInOwl:hasOBONamespace>
        <oboInOwl:id>GAZ:00080263</oboInOwl:id>
        <rdfs:label>Chattar Subdistrict</rdfs:label>
    </owl:NamedIndividual>
    


    <!-- http://purl.obolibrary.org/obo/GAZ_00080264 -->

    <owl:NamedIndividual rdf:about="http://purl.obolibrary.org/obo/GAZ_00080264">
        <obo:RO_0001025 rdf:resource="http://purl.obolibrary.org/obo/GAZ_00400014"/>
        <obo:IAO_0000115>A Subdistrict of Panjgur District, Balochistan.</obo:IAO_0000115>
        <oboInOwl:hasOBONamespace>GAZ</oboInOwl:hasOBONamespace>
        <oboInOwl:id>GAZ:00080264</oboInOwl:id>
        <rdfs:label>Panjgur Subdistrict</rdfs:label>
    </owl:NamedIndividual>
    


    <!-- http://purl.obolibrary.org/obo/GAZ_00080265 -->

    <owl:NamedIndividual rdf:about="http://purl.obolibrary.org/obo/GAZ_00080265">
        <obo:RO_0001025 rdf:resource="http://purl.obolibrary.org/obo/GAZ_00080264"/>
        <obo:IAO_0000115>A Sub-Tehsil of Panjgur District, Balochistan.</obo:IAO_0000115>
        <oboInOwl:hasOBONamespace>GAZ</oboInOwl:hasOBONamespace>
        <oboInOwl:id>GAZ:00080265</oboInOwl:id>
        <rdfs:label>Parome Sub-Tehsil</rdfs:label>
    </owl:NamedIndividual>
    


    <!-- http://purl.obolibrary.org/obo/GAZ_00080266 -->

    <owl:NamedIndividual rdf:about="http://purl.obolibrary.org/obo/GAZ_00080266">
        <obo:RO_0001025 rdf:resource="http://purl.obolibrary.org/obo/GAZ_00080264"/>
        <obo:IAO_0000115>A Sub-Tehsil of Panjgur District, Balochistan.</obo:IAO_0000115>
        <oboInOwl:hasOBONamespace>GAZ</oboInOwl:hasOBONamespace>
        <oboInOwl:id>GAZ:00080266</oboInOwl:id>
        <rdfs:label>Gichk Sub-Tehsil</rdfs:label>
    </owl:NamedIndividual>
    


    <!-- http://purl.obolibrary.org/obo/GAZ_00080267 -->

    <owl:NamedIndividual rdf:about="http://purl.obolibrary.org/obo/GAZ_00080267">
        <obo:RO_0001025 rdf:resource="http://purl.obolibrary.org/obo/GAZ_00080264"/>
        <obo:IAO_0000115>A Tehsil of Panjgur District, Balochistan.</obo:IAO_0000115>
        <oboInOwl:hasOBONamespace>GAZ</oboInOwl:hasOBONamespace>
        <oboInOwl:id>GAZ:00080267</oboInOwl:id>
        <rdfs:label>Panjgur Tehsil</rdfs:label>
    </owl:NamedIndividual>
    


    <!-- http://purl.obolibrary.org/obo/GAZ_00080268 -->

    <owl:NamedIndividual rdf:about="http://purl.obolibrary.org/obo/GAZ_00080268">
        <obo:RO_0001025 rdf:resource="http://purl.obolibrary.org/obo/GAZ_00400009"/>
        <obo:IAO_0000115>A Tehsil in Pishin District, Balochistan.</obo:IAO_0000115>
        <oboInOwl:hasOBONamespace>GAZ</oboInOwl:hasOBONamespace>
        <oboInOwl:id>GAZ:00080268</oboInOwl:id>
        <rdfs:label>Barshore Tehsil</rdfs:label>
    </owl:NamedIndividual>
    


    <!-- http://purl.obolibrary.org/obo/GAZ_00080269 -->

    <owl:NamedIndividual rdf:about="http://purl.obolibrary.org/obo/GAZ_00080269">
        <obo:RO_0001025 rdf:resource="http://purl.obolibrary.org/obo/GAZ_00400009"/>
        <obo:IAO_0000115>A Tehsil in Pishin District, Balochistan.</obo:IAO_0000115>
        <oboInOwl:hasOBONamespace>GAZ</oboInOwl:hasOBONamespace>
        <oboInOwl:id>GAZ:00080269</oboInOwl:id>
        <rdfs:label>Bostan Tehsil</rdfs:label>
    </owl:NamedIndividual>
    


    <!-- http://purl.obolibrary.org/obo/GAZ_00080270 -->

    <owl:NamedIndividual rdf:about="http://purl.obolibrary.org/obo/GAZ_00080270">
        <obo:RO_0001025 rdf:resource="http://purl.obolibrary.org/obo/GAZ_00400009"/>
        <obo:IAO_0000115>A Tehsil in Pishin District, Balochistan.</obo:IAO_0000115>
        <oboInOwl:hasOBONamespace>GAZ</oboInOwl:hasOBONamespace>
        <oboInOwl:id>GAZ:00080270</oboInOwl:id>
        <rdfs:label>Pishin Tehsil</rdfs:label>
    </owl:NamedIndividual>
    


    <!-- http://purl.obolibrary.org/obo/GAZ_00080271 -->

    <owl:NamedIndividual rdf:about="http://purl.obolibrary.org/obo/GAZ_00080271">
        <obo:RO_0001025 rdf:resource="http://purl.obolibrary.org/obo/GAZ_00400009"/>
        <obo:IAO_0000115>A Tehsil in Pishin District, Balochistan.</obo:IAO_0000115>
        <oboInOwl:hasOBONamespace>GAZ</oboInOwl:hasOBONamespace>
        <oboInOwl:id>GAZ:00080271</oboInOwl:id>
        <rdfs:label>Karezat Tehsil</rdfs:label>
    </owl:NamedIndividual>
    


    <!-- http://purl.obolibrary.org/obo/GAZ_00080272 -->

    <owl:NamedIndividual rdf:about="http://purl.obolibrary.org/obo/GAZ_00080272">
        <obo:RO_0001025 rdf:resource="http://purl.obolibrary.org/obo/GAZ_00400009"/>
        <obo:IAO_0000115>A Tehsil in Pishin District, Balochistan.</obo:IAO_0000115>
        <oboInOwl:hasOBONamespace>GAZ</oboInOwl:hasOBONamespace>
        <oboInOwl:id>GAZ:00080272</oboInOwl:id>
        <rdfs:label>Hurramzai Tehsil</rdfs:label>
    </owl:NamedIndividual>
    


    <!-- http://purl.obolibrary.org/obo/GAZ_00080273 -->

    <owl:NamedIndividual rdf:about="http://purl.obolibrary.org/obo/GAZ_00080273">
        <obo:RO_0001025 rdf:resource="http://purl.obolibrary.org/obo/GAZ_00400010"/>
        <obo:IAO_0000115>A Subdistrict of Zhob District, Balocghistan.</obo:IAO_0000115>
        <oboInOwl:hasOBONamespace>GAZ</oboInOwl:hasOBONamespace>
        <oboInOwl:id>GAZ:00080273</oboInOwl:id>
        <rdfs:label>Zhob Subdistrict</rdfs:label>
    </owl:NamedIndividual>
    


    <!-- http://purl.obolibrary.org/obo/GAZ_00080274 -->

    <owl:NamedIndividual rdf:about="http://purl.obolibrary.org/obo/GAZ_00080274">
        <obo:RO_0001025 rdf:resource="http://purl.obolibrary.org/obo/GAZ_00400010"/>
        <obo:IAO_0000115>A Sub-Tehsil of Zhob District, Balochistan.</obo:IAO_0000115>
        <oboInOwl:hasOBONamespace>GAZ</oboInOwl:hasOBONamespace>
        <oboInOwl:id>GAZ:00080274</oboInOwl:id>
        <rdfs:label>Kakkar Subdistrct</rdfs:label>
    </owl:NamedIndividual>
    


    <!-- http://purl.obolibrary.org/obo/GAZ_00080275 -->

    <owl:NamedIndividual rdf:about="http://purl.obolibrary.org/obo/GAZ_00080275">
        <obo:RO_0001025 rdf:resource="http://purl.obolibrary.org/obo/GAZ_00400005"/>
        <oboInOwl:hasOBONamespace>GAZ</oboInOwl:hasOBONamespace>
        <oboInOwl:id>GAZ:00080275</oboInOwl:id>
        <rdfs:label>Sibi Tehsil</rdfs:label>
    </owl:NamedIndividual>
    


    <!-- http://purl.obolibrary.org/obo/GAZ_00080276 -->

    <owl:NamedIndividual rdf:about="http://purl.obolibrary.org/obo/GAZ_00080276">
        <obo:RO_0001025 rdf:resource="http://purl.obolibrary.org/obo/GAZ_00400005"/>
        <oboInOwl:hasOBONamespace>GAZ</oboInOwl:hasOBONamespace>
        <oboInOwl:id>GAZ:00080276</oboInOwl:id>
        <rdfs:label>Harnai Tehsil</rdfs:label>
    </owl:NamedIndividual>
    


    <!-- http://purl.obolibrary.org/obo/GAZ_00080277 -->

    <owl:NamedIndividual rdf:about="http://purl.obolibrary.org/obo/GAZ_00080277">
        <obo:RO_0001025 rdf:resource="http://purl.obolibrary.org/obo/GAZ_00400010"/>
        <obo:IAO_0000115>A Subdistrict of Zhob District, Balochistan province of Pakistan.</obo:IAO_0000115>
        <oboInOwl:hasOBONamespace>GAZ</oboInOwl:hasOBONamespace>
        <oboInOwl:id>GAZ:00080277</oboInOwl:id>
        <rdfs:label>Sherani Subdistrict</rdfs:label>
    </owl:NamedIndividual>
    


    <!-- http://purl.obolibrary.org/obo/GAZ_00080278 -->

    <owl:NamedIndividual rdf:about="http://purl.obolibrary.org/obo/GAZ_00080278">
        <obo:RO_0001025 rdf:resource="http://purl.obolibrary.org/obo/GAZ_00400005"/>
        <oboInOwl:hasOBONamespace>GAZ</oboInOwl:hasOBONamespace>
        <oboInOwl:id>GAZ:00080278</oboInOwl:id>
        <rdfs:label>Lehri Tehsil</rdfs:label>
    </owl:NamedIndividual>
    


    <!-- http://purl.obolibrary.org/obo/GAZ_00080279 -->

    <owl:NamedIndividual rdf:about="http://purl.obolibrary.org/obo/GAZ_00080279">
        <obo:RO_0001025 rdf:resource="http://purl.obolibrary.org/obo/GAZ_00080277"/>
        <obo:IAO_0000115>A Sub-Tehsil of Zhib District, Balochistan.</obo:IAO_0000115>
        <oboInOwl:hasOBONamespace>GAZ</oboInOwl:hasOBONamespace>
        <oboInOwl:id>GAZ:00080279</oboInOwl:id>
        <rdfs:label>Sherani Sub-Tehsil</rdfs:label>
    </owl:NamedIndividual>
    


    <!-- http://purl.obolibrary.org/obo/GAZ_00080280 -->

    <owl:NamedIndividual rdf:about="http://purl.obolibrary.org/obo/GAZ_00080280">
        <obo:RO_0001025 rdf:resource="http://purl.obolibrary.org/obo/GAZ_00080273"/>
        <obo:IAO_0000115>A Tehsil of Zhob District, Balochistan.</obo:IAO_0000115>
        <oboInOwl:hasOBONamespace>GAZ</oboInOwl:hasOBONamespace>
        <oboInOwl:id>GAZ:00080280</oboInOwl:id>
        <rdfs:label>Zhob Tehsil</rdfs:label>
    </owl:NamedIndividual>
    


    <!-- http://purl.obolibrary.org/obo/GAZ_00080281 -->

    <owl:NamedIndividual rdf:about="http://purl.obolibrary.org/obo/GAZ_00080281">
        <obo:RO_0001025 rdf:resource="http://purl.obolibrary.org/obo/GAZ_00400010"/>
        <obo:IAO_0000115>A Sub-Tehsil of Zhob District, Balochistan.</obo:IAO_0000115>
        <oboInOwl:hasOBONamespace>GAZ</oboInOwl:hasOBONamespace>
        <oboInOwl:id>GAZ:00080281</oboInOwl:id>
        <rdfs:label>Ashwat Sub-Tehsil</rdfs:label>
    </owl:NamedIndividual>
    


    <!-- http://purl.obolibrary.org/obo/GAZ_00080282 -->

    <owl:NamedIndividual rdf:about="http://purl.obolibrary.org/obo/GAZ_00080282">
        <obo:RO_0001025 rdf:resource="http://purl.obolibrary.org/obo/GAZ_00400010"/>
        <obo:IAO_0000115>A Tehsil of Zhob District, Balochistan ?</obo:IAO_0000115>
        <oboInOwl:hasOBONamespace>GAZ</oboInOwl:hasOBONamespace>
        <oboInOwl:id>GAZ:00080282</oboInOwl:id>
        <rdfs:label>Qamar Din Karez</rdfs:label>
    </owl:NamedIndividual>
    


    <!-- http://purl.obolibrary.org/obo/GAZ_00080283 -->

    <owl:NamedIndividual rdf:about="http://purl.obolibrary.org/obo/GAZ_00080283">
        <obo:RO_0001025 rdf:resource="http://purl.obolibrary.org/obo/GAZ_00400010"/>
        <obo:IAO_0000115>A Sub-Tehsil of Zhob District, Balochistan.</obo:IAO_0000115>
        <oboInOwl:hasOBONamespace>GAZ</oboInOwl:hasOBONamespace>
        <oboInOwl:id>GAZ:00080283</oboInOwl:id>
        <rdfs:label>Sambaza Sub-Tehsil</rdfs:label>
    </owl:NamedIndividual>
    


    <!-- http://purl.obolibrary.org/obo/GAZ_00080284 -->

    <owl:NamedIndividual rdf:about="http://purl.obolibrary.org/obo/GAZ_00080284">
        <obo:RO_0001025 rdf:resource="http://purl.obolibrary.org/obo/GAZ_00400001"/>
        <obo:IAO_0000115>A Tehsil of Ziarit District, Balochistan.</obo:IAO_0000115>
        <oboInOwl:hasOBONamespace>GAZ</oboInOwl:hasOBONamespace>
        <oboInOwl:id>GAZ:00080284</oboInOwl:id>
        <rdfs:label>Ziarat Tehsil</rdfs:label>
    </owl:NamedIndividual>
    


    <!-- http://purl.obolibrary.org/obo/GAZ_00080285 -->

    <owl:NamedIndividual rdf:about="http://purl.obolibrary.org/obo/GAZ_00080285">
        <obo:RO_0001025 rdf:resource="http://purl.obolibrary.org/obo/GAZ_00400001"/>
        <obo:IAO_0000115>A Tehsil of Ziarit District, Balochistan.</obo:IAO_0000115>
        <oboInOwl:hasOBONamespace>GAZ</oboInOwl:hasOBONamespace>
        <oboInOwl:id>GAZ:00080285</oboInOwl:id>
        <rdfs:label>Sinjavi Tehsil</rdfs:label>
    </owl:NamedIndividual>
    


    <!-- http://purl.obolibrary.org/obo/GAZ_00080286 -->

    <owl:NamedIndividual rdf:about="http://purl.obolibrary.org/obo/GAZ_00080286">
        <rdf:type rdf:resource="http://purl.obolibrary.org/obo/ENVO_00000856"/>
        <obo:RO_0001025 rdf:resource="http://purl.obolibrary.org/obo/GAZ_00007411"/>
        <obo:IAO_0000115>A populated place. A town located in the western part of Karachi, Sindh, Pakistan. It is bordered by SITE Town and Orangi to the east and by Kiamari Town to the north and west, with most of the western boundary formed by part of the RCD Highway.</obo:IAO_0000115>
        <oboInOwl:hasOBONamespace>GAZ</oboInOwl:hasOBONamespace>
        <oboInOwl:id>GAZ:00080286</oboInOwl:id>
        <rdfs:label>Baldia Town</rdfs:label>
    </owl:NamedIndividual>
    


    <!-- http://purl.obolibrary.org/obo/GAZ_00080287 -->

    <owl:NamedIndividual rdf:about="http://purl.obolibrary.org/obo/GAZ_00080287">
        <rdf:type rdf:resource="http://purl.obolibrary.org/obo/ENVO_00000856"/>
        <obo:RO_0001025 rdf:resource="http://purl.obolibrary.org/obo/GAZ_00007411"/>
        <obo:IAO_0000115>A populated place. A town located in the southeastern part of Karachi along the Arabian Sea and the Indus River delta. Bin Qasim is bordered by Gadap Town to the north, Thatta District and the Indus River to the east, the Arabian Sea to the south and the Malir River and the towns of Landhi, Malir, and Korangi Cantonment to the west.</obo:IAO_0000115>
        <oboInOwl:hasOBONamespace>GAZ</oboInOwl:hasOBONamespace>
        <oboInOwl:id>GAZ:00080287</oboInOwl:id>
        <rdfs:label>Bin Qasim Town</rdfs:label>
    </owl:NamedIndividual>
    


    <!-- http://purl.obolibrary.org/obo/GAZ_00080288 -->

    <owl:NamedIndividual rdf:about="http://purl.obolibrary.org/obo/GAZ_00080288">
        <rdf:type rdf:resource="http://purl.obolibrary.org/obo/ENVO_00000856"/>
        <obo:RO_0001025 rdf:resource="http://purl.obolibrary.org/obo/GAZ_00007411"/>
        <obo:IAO_0000115>A populated place. A town located in the northwestern part of Karachi with the Hub River on its western limits also forming the provincial border between Sindh and Balochistan, while to the north and east are Dadu District and the Kirthar Mountains.</obo:IAO_0000115>
        <oboInOwl:hasOBONamespace>GAZ</oboInOwl:hasOBONamespace>
        <oboInOwl:id>GAZ:00080288</oboInOwl:id>
        <rdfs:label>Gadap Town</rdfs:label>
    </owl:NamedIndividual>
    


    <!-- http://purl.obolibrary.org/obo/GAZ_00080289 -->

    <owl:NamedIndividual rdf:about="http://purl.obolibrary.org/obo/GAZ_00080289">
        <obo:RO_0001025 rdf:resource="http://purl.obolibrary.org/obo/GAZ_00007411"/>
        <obo:IAO_0000115>One of the towns of Karachi, Pakistan. Georaphically it is situated in the northern part of the city but previously fell in the jurisdiction of District Central. Gulberg is bordered by the Lyari River and Gulshan Town to the east and the Gujar Nala stream and North Nazimabad Town to the west. Also neighbouring Gulberg are New Karachi and Gadap to the north and Liaquatabad to the south.</obo:IAO_0000115>
        <oboInOwl:hasOBONamespace>GAZ</oboInOwl:hasOBONamespace>
        <oboInOwl:id>GAZ:00080289</oboInOwl:id>
        <rdfs:label>Gulberg Town</rdfs:label>
    </owl:NamedIndividual>
    


    <!-- http://purl.obolibrary.org/obo/GAZ_00080290 -->

    <owl:NamedIndividual rdf:about="http://purl.obolibrary.org/obo/GAZ_00080290">
        <obo:RO_0001025 rdf:resource="http://purl.obolibrary.org/obo/GAZ_00007411"/>
        <obo:IAO_0000115>One of the towns in Karachi, Sindh, Pakistan. The town is bordered by Gadap Town to the north, the Faisal and Malir Cantonments to the east, Jamshed Town to the southwest, and Gulberg and Liaquatabad to the west.</obo:IAO_0000115>
        <oboInOwl:hasOBONamespace>GAZ</oboInOwl:hasOBONamespace>
        <oboInOwl:id>GAZ:00080290</oboInOwl:id>
        <rdfs:label>Gulshan Town</rdfs:label>
    </owl:NamedIndividual>
    


    <!-- http://purl.obolibrary.org/obo/GAZ_00080291 -->

    <owl:NamedIndividual rdf:about="http://purl.obolibrary.org/obo/GAZ_00080291">
        <obo:RO_0001025 rdf:resource="http://purl.obolibrary.org/obo/GAZ_00007411"/>
        <obo:IAO_0000115>The largest of the towns in Karachi, Sindh, Pakistan and lies in the central part of Karachi. To the northwest is Liaquatabad Town across the Lyari River, while to the east is Gulshan Town and to the southeast is Korangi Town across the Malir River. Jamshed is bordered by Karachi Cantonment and Clifton Cantonment to the west.</obo:IAO_0000115>
        <oboInOwl:hasOBONamespace>GAZ</oboInOwl:hasOBONamespace>
        <oboInOwl:id>GAZ:00080291</oboInOwl:id>
        <rdfs:label>Jamshed Town</rdfs:label>
    </owl:NamedIndividual>
    


    <!-- http://purl.obolibrary.org/obo/GAZ_00080292 -->

    <owl:NamedIndividual rdf:about="http://purl.obolibrary.org/obo/GAZ_00080292">
        <rdf:type rdf:resource="http://purl.obolibrary.org/obo/ENVO_00000856"/>
        <obo:RO_0001025 rdf:resource="http://purl.obolibrary.org/obo/GAZ_00007411"/>
        <obo:IAO_0000115>A populated place. A town in the eastern parts of Karachi, Pakistan, south of the Malir River. It is bordered by Faisal Cantonment and Shah Faisal Town to the north, Bin Qasim and Landhi to the east and south, Korangi Cantonment to the southwest and Jamshed Town to the west across the Malir River.</obo:IAO_0000115>
        <oboInOwl:hasOBONamespace>GAZ</oboInOwl:hasOBONamespace>
        <oboInOwl:id>GAZ:00080292</oboInOwl:id>
        <rdfs:label>Korangi Town</rdfs:label>
    </owl:NamedIndividual>
    


    <!-- http://purl.obolibrary.org/obo/GAZ_00080293 -->

    <owl:NamedIndividual rdf:about="http://purl.obolibrary.org/obo/GAZ_00080293">
        <obo:RO_0001025 rdf:resource="http://purl.obolibrary.org/obo/GAZ_00080292"/>
        <obo:RO_0001025 rdf:resource="http://purl.obolibrary.org/obo/GAZ_00253159"/>
        <obo:IAO_0000115>A harbor located in Karachi, Sindh, Pakistan.</obo:IAO_0000115>
        <oboInOwl:hasOBONamespace>GAZ</oboInOwl:hasOBONamespace>
        <oboInOwl:id>GAZ:00080293</oboInOwl:id>
        <rdfs:label>Korangi Fish Harbour</rdfs:label>
    </owl:NamedIndividual>
    


    <!-- http://purl.obolibrary.org/obo/GAZ_00080294 -->

    <owl:NamedIndividual rdf:about="http://purl.obolibrary.org/obo/GAZ_00080294">
        <obo:RO_0001025 rdf:resource="http://purl.obolibrary.org/obo/GAZ_00007411"/>
        <obo:IAO_0000115>A large industrial town in the eastern part of Karachi, Pakistan. It is bordered by the Faisal Cantonment and Shah Faisal Town to the north across the Malir River, Bin Qasim Town to the south and east, and Korangi Town to the west.</obo:IAO_0000115>
        <oboInOwl:hasOBONamespace>GAZ</oboInOwl:hasOBONamespace>
        <oboInOwl:id>GAZ:00080294</oboInOwl:id>
        <rdfs:label>Landhi Town</rdfs:label>
    </owl:NamedIndividual>
    


    <!-- http://purl.obolibrary.org/obo/GAZ_00080295 -->

    <owl:NamedIndividual rdf:about="http://purl.obolibrary.org/obo/GAZ_00080295">
        <rdf:type rdf:resource="http://purl.obolibrary.org/obo/ENVO_00000856"/>
        <obo:RO_0001025 rdf:resource="http://purl.obolibrary.org/obo/GAZ_00007411"/>
        <obo:IAO_0000115>A populated place. A town in the central part of Karachi, Pakistan. It is bordered by the towns of North Nazimabad to the north, Gulberg and Gulshan to the east, Jamshed to the south across the Lyari River, and SITE Town to the west across the Orangi Nala stream.</obo:IAO_0000115>
        <oboInOwl:hasOBONamespace>GAZ</oboInOwl:hasOBONamespace>
        <oboInOwl:id>GAZ:00080295</oboInOwl:id>
        <rdfs:label>Liaquatabad Town</rdfs:label>
    </owl:NamedIndividual>
    


    <!-- http://purl.obolibrary.org/obo/GAZ_00080296 -->

    <owl:NamedIndividual rdf:about="http://purl.obolibrary.org/obo/GAZ_00080296">
        <obo:RO_0001025 rdf:resource="http://purl.obolibrary.org/obo/GAZ_00007411"/>
        <obo:IAO_0000115>One of the eighteen constituent towns of the city of Karachi, in the province of Sindh, Pakistan. It is bordered by the towns of SITE Town to the north across the Lyari River, Jamshed and Saddar to the east, and Kiamari to the west across the main harbour of Karachi.</obo:IAO_0000115>
        <oboInOwl:hasOBONamespace>GAZ</oboInOwl:hasOBONamespace>
        <oboInOwl:id>GAZ:00080296</oboInOwl:id>
        <rdfs:label>Lyari Town</rdfs:label>
    </owl:NamedIndividual>
    


    <!-- http://purl.obolibrary.org/obo/GAZ_00080297 -->

    <owl:NamedIndividual rdf:about="http://purl.obolibrary.org/obo/GAZ_00080297">
        <obo:RO_0001025 rdf:resource="http://purl.obolibrary.org/obo/GAZ_00007411"/>
        <obo:IAO_0000115>A small densely populated town located in the Eastern part of Karachi, Sindh, Pakistan. Malir town bordered by Jinnah International Airport, Malir Cantonment to the West and North, the Malir River and Shah Faisal Town to the South and Gadap Town to the East across the Thado Nallo stream.</obo:IAO_0000115>
        <oboInOwl:hasOBONamespace>GAZ</oboInOwl:hasOBONamespace>
        <oboInOwl:id>GAZ:00080297</oboInOwl:id>
        <rdfs:label>Malir Town</rdfs:label>
    </owl:NamedIndividual>
    


    <!-- http://purl.obolibrary.org/obo/GAZ_00080298 -->

    <owl:NamedIndividual rdf:about="http://purl.obolibrary.org/obo/GAZ_00080298">
        <obo:RO_0001025 rdf:resource="http://purl.obolibrary.org/obo/GAZ_00007411"/>
        <obo:IAO_0000115>A small densely populated town in the northern part of Karachi, located between the Lyari River, the Manghopir Hills and two major roads - Surjani Road to the north and Shahrah-e-Zahid Hussain to the south. To the north and west lies the town of Gadap, and to the south lie the towns of Gulberg and North Nazimabad.</obo:IAO_0000115>
        <oboInOwl:hasOBONamespace>GAZ</oboInOwl:hasOBONamespace>
        <oboInOwl:id>GAZ:00080298</oboInOwl:id>
        <rdfs:label>New Karichi Town</rdfs:label>
    </owl:NamedIndividual>
    


    <!-- http://purl.obolibrary.org/obo/GAZ_00080299 -->

    <owl:NamedIndividual rdf:about="http://purl.obolibrary.org/obo/GAZ_00080299">
        <rdf:type rdf:resource="http://purl.obolibrary.org/obo/ENVO_00000856"/>
        <obo:RO_0001025 rdf:resource="http://purl.obolibrary.org/obo/GAZ_00007411"/>
        <obo:IAO_0000115>A populated place. A town in the northern part of Karachi, named as such in reference to it being north of the suburb of Nazimabad. The town is bordered by New Karachi Town to the north across the Shahrah-e-Zahid Hussain, Gulberg Town to the east across the Gujar Nala stream, Liaquatabad Town to the south, and SITE Town to the west.</obo:IAO_0000115>
        <oboInOwl:hasOBONamespace>GAZ</oboInOwl:hasOBONamespace>
        <oboInOwl:id>GAZ:00080299</oboInOwl:id>
        <rdfs:label>North Nazimabad Town</rdfs:label>
    </owl:NamedIndividual>
    


    <!-- http://purl.obolibrary.org/obo/GAZ_00080300 -->

    <owl:NamedIndividual rdf:about="http://purl.obolibrary.org/obo/GAZ_00080300">
        <obo:RO_0001025 rdf:resource="http://purl.obolibrary.org/obo/GAZ_00007411"/>
        <obo:IAO_0000115>A small densely populated town in the northwestern part of Karachi (Pakistan). It is bordered by New Karachi Town to the north across the Shahrah-e-Zahid Hussain, Gulberg Town to the east across the Gujar Nala stream, Liaquatabad Town to the south, and SITE Town to the west.</obo:IAO_0000115>
        <oboInOwl:hasOBONamespace>GAZ</oboInOwl:hasOBONamespace>
        <oboInOwl:id>GAZ:00080300</oboInOwl:id>
        <rdfs:label>Orangi Town</rdfs:label>
    </owl:NamedIndividual>
    


    <!-- http://purl.obolibrary.org/obo/GAZ_00080301 -->

    <owl:NamedIndividual rdf:about="http://purl.obolibrary.org/obo/GAZ_00080301">
        <obo:RO_0001025 rdf:resource="http://purl.obolibrary.org/obo/GAZ_00007411"/>
        <obo:IAO_0000115>A cantonment town of the city of Karachi, in Sindh, Pakistan. It serves as a military base and residential establishment. It was established by the British Indian Army in 19th century British India, and taken over by the Pakistan Army in 1947. The cantonment maintains its own infrastructure of water supply, electricity and is outside the jurisdiction of City District Government of Karachi.</obo:IAO_0000115>
        <oboInOwl:hasOBONamespace>GAZ</oboInOwl:hasOBONamespace>
        <oboInOwl:id>GAZ:00080301</oboInOwl:id>
        <rdfs:label>Clifton Cantonment</rdfs:label>
    </owl:NamedIndividual>
    


    <!-- http://purl.obolibrary.org/obo/GAZ_00080302 -->

    <owl:NamedIndividual rdf:about="http://purl.obolibrary.org/obo/GAZ_00080302">
        <obo:RO_0001025 rdf:resource="http://purl.obolibrary.org/obo/GAZ_00007411"/>
        <obo:IAO_0000115>A small, densely populated town in western part of Karachi, Pakistan and is named after the Sindh Industrial Trading Estate, which forms the heart of the town. The town is bordered by Gadap Town to the north, Liaquatabad and North Nazimabad to the east across the Orangi Nala stream, Lyari and Saddar to the south across the Lyari River and Kiamari to the west. Also neighbouring the town are Baldia and Orangi to the northwest.</obo:IAO_0000115>
        <oboInOwl:hasOBONamespace>GAZ</oboInOwl:hasOBONamespace>
        <oboInOwl:id>GAZ:00080302</oboInOwl:id>
        <rdfs:label>SITE Town</rdfs:label>
    </owl:NamedIndividual>
    


    <!-- http://purl.obolibrary.org/obo/GAZ_00080303 -->

    <owl:NamedIndividual rdf:about="http://purl.obolibrary.org/obo/GAZ_00080303">
        <obo:RO_0001025 rdf:resource="http://purl.obolibrary.org/obo/GAZ_00007411"/>
        <obo:IAO_0000115>A small, densely populated town in eastern Karachi. The town is bordered by Malir Town to the northeast, Bin Qasim Town to the east, Korangi Town and Landhi Town to the south, and Faisal Cantonment and Malir Cantonment to the west and northwest. The Malir River forms the southern boundary of the town and the Shahrah-e-Faisal highway forms much of the northern boundary with the Jinnah International Airport at the northern end of the town.</obo:IAO_0000115>
        <oboInOwl:hasOBONamespace>GAZ</oboInOwl:hasOBONamespace>
        <oboInOwl:id>GAZ:00080303</oboInOwl:id>
        <rdfs:label>Shah Faisal Town</rdfs:label>
    </owl:NamedIndividual>
    


    <!-- http://purl.obolibrary.org/obo/GAZ_00080304 -->

    <owl:NamedIndividual rdf:about="http://purl.obolibrary.org/obo/GAZ_00080304">
        <obo:RO_0001025 rdf:resource="http://purl.obolibrary.org/obo/GAZ_00007411"/>
        <obo:IAO_0000115>A cantonment in Karachi.</obo:IAO_0000115>
        <oboInOwl:hasOBONamespace>GAZ</oboInOwl:hasOBONamespace>
        <oboInOwl:id>GAZ:00080304</oboInOwl:id>
        <rdfs:label>Manora Cantonment</rdfs:label>
    </owl:NamedIndividual>
    


    <!-- http://purl.obolibrary.org/obo/GAZ_00080305 -->

    <owl:NamedIndividual rdf:about="http://purl.obolibrary.org/obo/GAZ_00080305">
        <obo:RO_0001025 rdf:resource="http://purl.obolibrary.org/obo/GAZ_00018553"/>
        <obo:IAO_0000115>A Tehsil (Taluka) of Larkano District, Sindh.</obo:IAO_0000115>
        <oboInOwl:hasOBONamespace>GAZ</oboInOwl:hasOBONamespace>
        <oboInOwl:id>GAZ:00080305</oboInOwl:id>
        <rdfs:label>Bakrani Taluka</rdfs:label>
    </owl:NamedIndividual>
    


    <!-- http://purl.obolibrary.org/obo/GAZ_00080306 -->

    <owl:NamedIndividual rdf:about="http://purl.obolibrary.org/obo/GAZ_00080306">
        <obo:RO_0001025 rdf:resource="http://purl.obolibrary.org/obo/GAZ_00018553"/>
        <obo:IAO_0000115>A Tehsil (Taluka) of Larkano District, Sindh.</obo:IAO_0000115>
        <oboInOwl:hasOBONamespace>GAZ</oboInOwl:hasOBONamespace>
        <oboInOwl:id>GAZ:00080306</oboInOwl:id>
        <rdfs:label>Dokri Taluka</rdfs:label>
    </owl:NamedIndividual>
    


    <!-- http://purl.obolibrary.org/obo/GAZ_00080307 -->

    <owl:NamedIndividual rdf:about="http://purl.obolibrary.org/obo/GAZ_00080307">
        <obo:RO_0001025 rdf:resource="http://purl.obolibrary.org/obo/GAZ_00018553"/>
        <obo:IAO_0000115>A Tehsil (Taluka) of Larkano District, Sindh.</obo:IAO_0000115>
        <oboInOwl:hasOBONamespace>GAZ</oboInOwl:hasOBONamespace>
        <oboInOwl:id>GAZ:00080307</oboInOwl:id>
        <rdfs:label>Ratodero Taluka</rdfs:label>
    </owl:NamedIndividual>
    


    <!-- http://purl.obolibrary.org/obo/GAZ_00080308 -->

    <owl:NamedIndividual rdf:about="http://purl.obolibrary.org/obo/GAZ_00080308">
        <obo:RO_0001025 rdf:resource="http://purl.obolibrary.org/obo/GAZ_00018553"/>
        <obo:IAO_0000115>A Tehsil (Taluka) of Larkano District, Sindh.</obo:IAO_0000115>
        <oboInOwl:hasOBONamespace>GAZ</oboInOwl:hasOBONamespace>
        <oboInOwl:id>GAZ:00080308</oboInOwl:id>
        <rdfs:label>Larkana Taluka</rdfs:label>
    </owl:NamedIndividual>
    


    <!-- http://purl.obolibrary.org/obo/GAZ_00080309 -->

    <owl:NamedIndividual rdf:about="http://purl.obolibrary.org/obo/GAZ_00080309">
        <obo:RO_0001025 rdf:resource="http://purl.obolibrary.org/obo/GAZ_00018545"/>
        <obo:IAO_0000115>A Tehsil (Taluka) of Jacobabad District, Sindh.</obo:IAO_0000115>
        <oboInOwl:hasOBONamespace>GAZ</oboInOwl:hasOBONamespace>
        <oboInOwl:id>GAZ:00080309</oboInOwl:id>
        <rdfs:label>Jacobabad Taluka</rdfs:label>
    </owl:NamedIndividual>
    


    <!-- http://purl.obolibrary.org/obo/GAZ_00080310 -->

    <owl:NamedIndividual rdf:about="http://purl.obolibrary.org/obo/GAZ_00080310">
        <obo:RO_0001025 rdf:resource="http://purl.obolibrary.org/obo/GAZ_00018545"/>
        <obo:IAO_0000115>A Tehsil (Taluka) of Jacobabad District, Sindh.</obo:IAO_0000115>
        <oboInOwl:hasOBONamespace>GAZ</oboInOwl:hasOBONamespace>
        <oboInOwl:id>GAZ:00080310</oboInOwl:id>
        <rdfs:label>Thull Taluka</rdfs:label>
    </owl:NamedIndividual>
    


    <!-- http://purl.obolibrary.org/obo/GAZ_00080311 -->

    <owl:NamedIndividual rdf:about="http://purl.obolibrary.org/obo/GAZ_00080311">
        <obo:RO_0001025 rdf:resource="http://purl.obolibrary.org/obo/GAZ_00018545"/>
        <obo:IAO_0000115>A Tehsil (Taluka) of Jacobabad District, Sindh.</obo:IAO_0000115>
        <oboInOwl:hasOBONamespace>GAZ</oboInOwl:hasOBONamespace>
        <oboInOwl:id>GAZ:00080311</oboInOwl:id>
        <rdfs:label>Khairo Taluka</rdfs:label>
    </owl:NamedIndividual>
    


    <!-- http://purl.obolibrary.org/obo/GAZ_00080312 -->

    <owl:NamedIndividual rdf:about="http://purl.obolibrary.org/obo/GAZ_00080312">
        <obo:RO_0001025 rdf:resource="http://purl.obolibrary.org/obo/GAZ_00018545"/>
        <obo:IAO_0000115>A Tehsil (Taluka) of Jacobabad District, Sindh.</obo:IAO_0000115>
        <oboInOwl:hasOBONamespace>GAZ</oboInOwl:hasOBONamespace>
        <oboInOwl:id>GAZ:00080312</oboInOwl:id>
        <rdfs:label>Ghari Khairo Taluka</rdfs:label>
    </owl:NamedIndividual>
    


    <!-- http://purl.obolibrary.org/obo/GAZ_00080313 -->

    <owl:NamedIndividual rdf:about="http://purl.obolibrary.org/obo/GAZ_00080313">
        <obo:RO_0001025 rdf:resource="http://purl.obolibrary.org/obo/GAZ_00018550"/>
        <obo:IAO_0000115>One of the four Talukas of Shikarpur, Sindh Province.</obo:IAO_0000115>
        <oboInOwl:hasOBONamespace>GAZ</oboInOwl:hasOBONamespace>
        <oboInOwl:id>GAZ:00080313</oboInOwl:id>
        <rdfs:label>Lakhi Taluka</rdfs:label>
    </owl:NamedIndividual>
    


    <!-- http://purl.obolibrary.org/obo/GAZ_00080314 -->

    <owl:NamedIndividual rdf:about="http://purl.obolibrary.org/obo/GAZ_00080314">
        <obo:RO_0001025 rdf:resource="http://purl.obolibrary.org/obo/GAZ_00018550"/>
        <obo:IAO_0000115>One of the four Talukas of Shikarpur, Sindh Province.</obo:IAO_0000115>
        <oboInOwl:hasOBONamespace>GAZ</oboInOwl:hasOBONamespace>
        <oboInOwl:id>GAZ:00080314</oboInOwl:id>
        <rdfs:label>Khan Pur Taluka</rdfs:label>
    </owl:NamedIndividual>
    


    <!-- http://purl.obolibrary.org/obo/GAZ_00080315 -->

    <owl:NamedIndividual rdf:about="http://purl.obolibrary.org/obo/GAZ_00080315">
        <obo:RO_0001025 rdf:resource="http://purl.obolibrary.org/obo/GAZ_00018550"/>
        <obo:IAO_0000115>One of the four Talukas of Shikarpur, Sindh Province.</obo:IAO_0000115>
        <oboInOwl:hasOBONamespace>GAZ</oboInOwl:hasOBONamespace>
        <oboInOwl:id>GAZ:00080315</oboInOwl:id>
        <rdfs:label>Shikarpur Taluka</rdfs:label>
    </owl:NamedIndividual>
    


    <!-- http://purl.obolibrary.org/obo/GAZ_00080316 -->

    <owl:NamedIndividual rdf:about="http://purl.obolibrary.org/obo/GAZ_00080316">
        <obo:RO_0001025 rdf:resource="http://purl.obolibrary.org/obo/GAZ_00018550"/>
        <obo:IAO_0000115>One of the four Talukas of Shikarpur, Sindh Province.</obo:IAO_0000115>
        <oboInOwl:hasOBONamespace>GAZ</oboInOwl:hasOBONamespace>
        <oboInOwl:id>GAZ:00080316</oboInOwl:id>
        <rdfs:label>Garhi Yaseen Taluka</rdfs:label>
    </owl:NamedIndividual>
    


    <!-- http://purl.obolibrary.org/obo/GAZ_00080317 -->

    <owl:NamedIndividual rdf:about="http://purl.obolibrary.org/obo/GAZ_00080317">
        <obo:RO_0001025 rdf:resource="http://purl.obolibrary.org/obo/GAZ_00018546"/>
        <obo:IAO_0000115>A Taluka in Qamber-Shahdad Kot District, Sindh.</obo:IAO_0000115>
        <oboInOwl:hasOBONamespace>GAZ</oboInOwl:hasOBONamespace>
        <oboInOwl:id>GAZ:00080317</oboInOwl:id>
        <rdfs:label>Miro Khan Taluka</rdfs:label>
    </owl:NamedIndividual>
    


    <!-- http://purl.obolibrary.org/obo/GAZ_00080318 -->

    <owl:NamedIndividual rdf:about="http://purl.obolibrary.org/obo/GAZ_00080318">
        <obo:RO_0001025 rdf:resource="http://purl.obolibrary.org/obo/GAZ_00018546"/>
        <obo:IAO_0000115>A Taluka in Qamber-Shahdad Kot District, Sindh.</obo:IAO_0000115>
        <oboInOwl:hasOBONamespace>GAZ</oboInOwl:hasOBONamespace>
        <oboInOwl:id>GAZ:00080318</oboInOwl:id>
        <rdfs:label>Kambar Taluka</rdfs:label>
    </owl:NamedIndividual>
    


    <!-- http://purl.obolibrary.org/obo/GAZ_00080319 -->

    <owl:NamedIndividual rdf:about="http://purl.obolibrary.org/obo/GAZ_00080319">
        <obo:RO_0001025 rdf:resource="http://purl.obolibrary.org/obo/GAZ_00018546"/>
        <obo:IAO_0000115>A Taluka in Qamber-Shahdad Kot District, Sindh.</obo:IAO_0000115>
        <oboInOwl:hasOBONamespace>GAZ</oboInOwl:hasOBONamespace>
        <oboInOwl:id>GAZ:00080319</oboInOwl:id>
        <rdfs:label>Shahdadkot Taluka</rdfs:label>
    </owl:NamedIndividual>
    


    <!-- http://purl.obolibrary.org/obo/GAZ_00080320 -->

    <owl:NamedIndividual rdf:about="http://purl.obolibrary.org/obo/GAZ_00080320">
        <obo:RO_0001025 rdf:resource="http://purl.obolibrary.org/obo/GAZ_00018553"/>
        <obo:IAO_0000115>A Tehsil (Taluka) of Larkano District, Sindh.</obo:IAO_0000115>
        <oboInOwl:hasOBONamespace>GAZ</oboInOwl:hasOBONamespace>
        <oboInOwl:id>GAZ:00080320</oboInOwl:id>
        <rdfs:label>Warah Takula</rdfs:label>
    </owl:NamedIndividual>
    


    <!-- http://purl.obolibrary.org/obo/GAZ_00080321 -->

    <owl:NamedIndividual rdf:about="http://purl.obolibrary.org/obo/GAZ_00080321">
        <obo:RO_0001025 rdf:resource="http://purl.obolibrary.org/obo/GAZ_00018548"/>
        <obo:IAO_0000115>A Taluka of Sukkur District in the Sindh province of Pakistan.</obo:IAO_0000115>
        <oboInOwl:hasOBONamespace>GAZ</oboInOwl:hasOBONamespace>
        <oboInOwl:id>GAZ:00080321</oboInOwl:id>
        <rdfs:label>Sukkur Taluka</rdfs:label>
    </owl:NamedIndividual>
    


    <!-- http://purl.obolibrary.org/obo/GAZ_00080322 -->

    <owl:NamedIndividual rdf:about="http://purl.obolibrary.org/obo/GAZ_00080322">
        <obo:RO_0001025 rdf:resource="http://purl.obolibrary.org/obo/GAZ_00018548"/>
        <obo:IAO_0000115>A Taluka of Sukkur District in the Sindh province of Pakistan.</obo:IAO_0000115>
        <oboInOwl:hasOBONamespace>GAZ</oboInOwl:hasOBONamespace>
        <oboInOwl:id>GAZ:00080322</oboInOwl:id>
        <rdfs:label>Rohri Taluka</rdfs:label>
    </owl:NamedIndividual>
    


    <!-- http://purl.obolibrary.org/obo/GAZ_00080323 -->

    <owl:NamedIndividual rdf:about="http://purl.obolibrary.org/obo/GAZ_00080323">
        <obo:RO_0001025 rdf:resource="http://purl.obolibrary.org/obo/GAZ_00400084"/>
        <obo:IAO_0000115>A Taluka in Tando Allah Yaar District, Sindh.</obo:IAO_0000115>
        <oboInOwl:hasOBONamespace>GAZ</oboInOwl:hasOBONamespace>
        <oboInOwl:id>GAZ:00080323</oboInOwl:id>
        <rdfs:label>Chamber Taluka</rdfs:label>
    </owl:NamedIndividual>
    


    <!-- http://purl.obolibrary.org/obo/GAZ_00080324 -->

    <owl:NamedIndividual rdf:about="http://purl.obolibrary.org/obo/GAZ_00080324">
        <obo:RO_0001025 rdf:resource="http://purl.obolibrary.org/obo/GAZ_00018548"/>
        <obo:IAO_0000115>A Taluka of Sukkur District in the Sindh province of Pakistan.</obo:IAO_0000115>
        <oboInOwl:hasOBONamespace>GAZ</oboInOwl:hasOBONamespace>
        <oboInOwl:id>GAZ:00080324</oboInOwl:id>
        <rdfs:label>Saleh Pat Taluka</rdfs:label>
    </owl:NamedIndividual>
    


    <!-- http://purl.obolibrary.org/obo/GAZ_00080325 -->

    <owl:NamedIndividual rdf:about="http://purl.obolibrary.org/obo/GAZ_00080325">
        <obo:RO_0001025 rdf:resource="http://purl.obolibrary.org/obo/GAZ_00018548"/>
        <obo:IAO_0000115>A Taluka of Sukkur District in the Sindh province of Pakistan.</obo:IAO_0000115>
        <oboInOwl:hasOBONamespace>GAZ</oboInOwl:hasOBONamespace>
        <oboInOwl:id>GAZ:00080325</oboInOwl:id>
        <rdfs:label>Pano Akil Taluka</rdfs:label>
    </owl:NamedIndividual>
    


    <!-- http://purl.obolibrary.org/obo/GAZ_00080326 -->

    <owl:NamedIndividual rdf:about="http://purl.obolibrary.org/obo/GAZ_00080326">
        <obo:RO_0001025 rdf:resource="http://purl.obolibrary.org/obo/GAZ_00018554"/>
        <obo:IAO_0000115>A Taluka in Ghutki District, Sindh.</obo:IAO_0000115>
        <oboInOwl:hasOBONamespace>GAZ</oboInOwl:hasOBONamespace>
        <oboInOwl:id>GAZ:00080326</oboInOwl:id>
        <rdfs:label>Mirpur Mathelo Taluka</rdfs:label>
    </owl:NamedIndividual>
    


    <!-- http://purl.obolibrary.org/obo/GAZ_00080327 -->

    <owl:NamedIndividual rdf:about="http://purl.obolibrary.org/obo/GAZ_00080327">
        <obo:RO_0001025 rdf:resource="http://purl.obolibrary.org/obo/GAZ_00018554"/>
        <obo:IAO_0000115>A Taluka in Ghutki District, Sindh.</obo:IAO_0000115>
        <oboInOwl:hasOBONamespace>GAZ</oboInOwl:hasOBONamespace>
        <oboInOwl:id>GAZ:00080327</oboInOwl:id>
        <rdfs:label>Khan Garh Taluka</rdfs:label>
    </owl:NamedIndividual>
    


    <!-- http://purl.obolibrary.org/obo/GAZ_00080328 -->

    <owl:NamedIndividual rdf:about="http://purl.obolibrary.org/obo/GAZ_00080328">
        <obo:RO_0001025 rdf:resource="http://purl.obolibrary.org/obo/GAZ_00018554"/>
        <obo:IAO_0000115>A Taluka in Ghutki District, Sindh.</obo:IAO_0000115>
        <oboInOwl:hasOBONamespace>GAZ</oboInOwl:hasOBONamespace>
        <oboInOwl:id>GAZ:00080328</oboInOwl:id>
        <rdfs:label>Ghotki Taluka</rdfs:label>
    </owl:NamedIndividual>
    


    <!-- http://purl.obolibrary.org/obo/GAZ_00080329 -->

    <owl:NamedIndividual rdf:about="http://purl.obolibrary.org/obo/GAZ_00080329">
        <obo:RO_0001025 rdf:resource="http://purl.obolibrary.org/obo/GAZ_00018554"/>
        <obo:IAO_0000115>A Taluka in Ghutki District, Sindh.</obo:IAO_0000115>
        <oboInOwl:hasOBONamespace>GAZ</oboInOwl:hasOBONamespace>
        <oboInOwl:id>GAZ:00080329</oboInOwl:id>
        <rdfs:label>Ubauro Taluka</rdfs:label>
    </owl:NamedIndividual>
    


    <!-- http://purl.obolibrary.org/obo/GAZ_00080330 -->

    <owl:NamedIndividual rdf:about="http://purl.obolibrary.org/obo/GAZ_00080330">
        <obo:RO_0001025 rdf:resource="http://purl.obolibrary.org/obo/GAZ_00400092"/>
        <obo:IAO_0000115>A Taluka in Kashmor District, Sindh.</obo:IAO_0000115>
        <oboInOwl:hasOBONamespace>GAZ</oboInOwl:hasOBONamespace>
        <oboInOwl:id>GAZ:00080330</oboInOwl:id>
        <rdfs:label>Kashmore Taluka</rdfs:label>
    </owl:NamedIndividual>
    


    <!-- http://purl.obolibrary.org/obo/GAZ_00080331 -->

    <owl:NamedIndividual rdf:about="http://purl.obolibrary.org/obo/GAZ_00080331">
        <obo:RO_0001025 rdf:resource="http://purl.obolibrary.org/obo/GAZ_00400092"/>
        <obo:IAO_0000115>A Taluka in Kashmor District, Sindh.</obo:IAO_0000115>
        <oboInOwl:hasOBONamespace>GAZ</oboInOwl:hasOBONamespace>
        <oboInOwl:id>GAZ:00080331</oboInOwl:id>
        <rdfs:label>Kandhkot Taluka</rdfs:label>
    </owl:NamedIndividual>
    


    <!-- http://purl.obolibrary.org/obo/GAZ_00080332 -->

    <owl:NamedIndividual rdf:about="http://purl.obolibrary.org/obo/GAZ_00080332">
        <obo:RO_0001025 rdf:resource="http://purl.obolibrary.org/obo/GAZ_00400092"/>
        <obo:IAO_0000115>A Taluka in Kashmor District, Sindh.</obo:IAO_0000115>
        <oboInOwl:hasOBONamespace>GAZ</oboInOwl:hasOBONamespace>
        <oboInOwl:id>GAZ:00080332</oboInOwl:id>
        <rdfs:label>Tangwani Taluka</rdfs:label>
    </owl:NamedIndividual>
    


    <!-- http://purl.obolibrary.org/obo/GAZ_00080333 -->

    <owl:NamedIndividual rdf:about="http://purl.obolibrary.org/obo/GAZ_00080333">
        <obo:RO_0001025 rdf:resource="http://purl.obolibrary.org/obo/GAZ_00018549"/>
        <obo:IAO_0000115>A Taluka of Khairpur District, Sindh.</obo:IAO_0000115>
        <oboInOwl:hasOBONamespace>GAZ</oboInOwl:hasOBONamespace>
        <oboInOwl:id>GAZ:00080333</oboInOwl:id>
        <rdfs:label>Kot Diji Taluka</rdfs:label>
    </owl:NamedIndividual>
    


    <!-- http://purl.obolibrary.org/obo/GAZ_00080334 -->

    <owl:NamedIndividual rdf:about="http://purl.obolibrary.org/obo/GAZ_00080334">
        <obo:RO_0001025 rdf:resource="http://purl.obolibrary.org/obo/GAZ_00018549"/>
        <obo:IAO_0000115>A Taluka of Khairpur District, Sindh.</obo:IAO_0000115>
        <oboInOwl:hasOBONamespace>GAZ</oboInOwl:hasOBONamespace>
        <oboInOwl:id>GAZ:00080334</oboInOwl:id>
        <rdfs:label>Faiz Ganj Taluka</rdfs:label>
    </owl:NamedIndividual>
    


    <!-- http://purl.obolibrary.org/obo/GAZ_00080335 -->

    <owl:NamedIndividual rdf:about="http://purl.obolibrary.org/obo/GAZ_00080335">
        <obo:RO_0001025 rdf:resource="http://purl.obolibrary.org/obo/GAZ_00018549"/>
        <obo:IAO_0000115>A Taluka of Khairpur District, Sindh.</obo:IAO_0000115>
        <oboInOwl:hasOBONamespace>GAZ</oboInOwl:hasOBONamespace>
        <oboInOwl:id>GAZ:00080335</oboInOwl:id>
        <rdfs:label>Gambat Taluka</rdfs:label>
    </owl:NamedIndividual>
    


    <!-- http://purl.obolibrary.org/obo/GAZ_00080336 -->

    <owl:NamedIndividual rdf:about="http://purl.obolibrary.org/obo/GAZ_00080336">
        <obo:RO_0001025 rdf:resource="http://purl.obolibrary.org/obo/GAZ_00018549"/>
        <obo:IAO_0000115>A Taluka of Khairpur District, Sindh.</obo:IAO_0000115>
        <oboInOwl:hasOBONamespace>GAZ</oboInOwl:hasOBONamespace>
        <oboInOwl:id>GAZ:00080336</oboInOwl:id>
        <rdfs:label>Kingri Taluka</rdfs:label>
    </owl:NamedIndividual>
    


    <!-- http://purl.obolibrary.org/obo/GAZ_00080337 -->

    <owl:NamedIndividual rdf:about="http://purl.obolibrary.org/obo/GAZ_00080337">
        <obo:RO_0001025 rdf:resource="http://purl.obolibrary.org/obo/GAZ_00018549"/>
        <obo:IAO_0000115>A Taluka of Khairpur District, Sindh.</obo:IAO_0000115>
        <oboInOwl:hasOBONamespace>GAZ</oboInOwl:hasOBONamespace>
        <oboInOwl:id>GAZ:00080337</oboInOwl:id>
        <rdfs:label>Nara Taluka</rdfs:label>
    </owl:NamedIndividual>
    


    <!-- http://purl.obolibrary.org/obo/GAZ_00080338 -->

    <owl:NamedIndividual rdf:about="http://purl.obolibrary.org/obo/GAZ_00080338">
        <obo:RO_0001025 rdf:resource="http://purl.obolibrary.org/obo/GAZ_00018549"/>
        <obo:IAO_0000115>A Taluka of Khairpur District, Sindh.</obo:IAO_0000115>
        <oboInOwl:hasOBONamespace>GAZ</oboInOwl:hasOBONamespace>
        <oboInOwl:id>GAZ:00080338</oboInOwl:id>
        <rdfs:label>Sobho Dero Taluka</rdfs:label>
    </owl:NamedIndividual>
    


    <!-- http://purl.obolibrary.org/obo/GAZ_00080339 -->

    <owl:NamedIndividual rdf:about="http://purl.obolibrary.org/obo/GAZ_00080339">
        <obo:RO_0001025 rdf:resource="http://purl.obolibrary.org/obo/GAZ_00018549"/>
        <obo:IAO_0000115>A Taluka of Khairpur District, Sindh.</obo:IAO_0000115>
        <oboInOwl:hasOBONamespace>GAZ</oboInOwl:hasOBONamespace>
        <oboInOwl:id>GAZ:00080339</oboInOwl:id>
        <rdfs:label>Khairpur Taluka</rdfs:label>
    </owl:NamedIndividual>
    


    <!-- http://purl.obolibrary.org/obo/GAZ_00080340 -->

    <owl:NamedIndividual rdf:about="http://purl.obolibrary.org/obo/GAZ_00080340">
        <obo:RO_0001025 rdf:resource="http://purl.obolibrary.org/obo/GAZ_00018549"/>
        <obo:IAO_0000115>A Taluka of Khairpur District, Sindh.</obo:IAO_0000115>
        <oboInOwl:hasOBONamespace>GAZ</oboInOwl:hasOBONamespace>
        <oboInOwl:id>GAZ:00080340</oboInOwl:id>
        <rdfs:label>Mirwah Taluka</rdfs:label>
    </owl:NamedIndividual>
    


    <!-- http://purl.obolibrary.org/obo/GAZ_00080341 -->

    <owl:NamedIndividual rdf:about="http://purl.obolibrary.org/obo/GAZ_00080341">
        <obo:RO_0001025 rdf:resource="http://purl.obolibrary.org/obo/GAZ_00400088"/>
        <obo:IAO_0000115>A Taluka of Jamshoro in the Sindh province of Pakistan.</obo:IAO_0000115>
        <oboInOwl:hasOBONamespace>GAZ</oboInOwl:hasOBONamespace>
        <oboInOwl:id>GAZ:00080341</oboInOwl:id>
        <rdfs:label>Sehwan Sharif Taluka</rdfs:label>
    </owl:NamedIndividual>
    


    <!-- http://purl.obolibrary.org/obo/GAZ_00080342 -->

    <owl:NamedIndividual rdf:about="http://purl.obolibrary.org/obo/GAZ_00080342">
        <obo:RO_0001025 rdf:resource="http://purl.obolibrary.org/obo/GAZ_00018552"/>
        <obo:IAO_0000115>A Taluka of Dadu District in the Sindh province of Pakistan.</obo:IAO_0000115>
        <oboInOwl:hasOBONamespace>GAZ</oboInOwl:hasOBONamespace>
        <oboInOwl:id>GAZ:00080342</oboInOwl:id>
        <rdfs:label>Dadu Taluka</rdfs:label>
    </owl:NamedIndividual>
    


    <!-- http://purl.obolibrary.org/obo/GAZ_00080343 -->

    <owl:NamedIndividual rdf:about="http://purl.obolibrary.org/obo/GAZ_00080343">
        <obo:RO_0001025 rdf:resource="http://purl.obolibrary.org/obo/GAZ_00018552"/>
        <obo:IAO_0000115>A Taluka of Dadu District in the Sindh province of Pakistan.</obo:IAO_0000115>
        <oboInOwl:hasOBONamespace>GAZ</oboInOwl:hasOBONamespace>
        <oboInOwl:id>GAZ:00080343</oboInOwl:id>
        <rdfs:label>Khairpur Nathan Shah Taluka</rdfs:label>
    </owl:NamedIndividual>
    


    <!-- http://purl.obolibrary.org/obo/GAZ_00080344 -->

    <owl:NamedIndividual rdf:about="http://purl.obolibrary.org/obo/GAZ_00080344">
        <obo:RO_0001025 rdf:resource="http://purl.obolibrary.org/obo/GAZ_00018552"/>
        <obo:IAO_0000115>A Taluka of Dadu District in the Sindh province of Pakistan.</obo:IAO_0000115>
        <oboInOwl:hasOBONamespace>GAZ</oboInOwl:hasOBONamespace>
        <oboInOwl:id>GAZ:00080344</oboInOwl:id>
        <rdfs:label>Mehar Taluka</rdfs:label>
    </owl:NamedIndividual>
    


    <!-- http://purl.obolibrary.org/obo/GAZ_00080345 -->

    <owl:NamedIndividual rdf:about="http://purl.obolibrary.org/obo/GAZ_00080345">
        <obo:RO_0001025 rdf:resource="http://purl.obolibrary.org/obo/GAZ_00018552"/>
        <obo:IAO_0000115>A Taluka of Dadu District in the Sindh province of Pakistan.</obo:IAO_0000115>
        <oboInOwl:hasOBONamespace>GAZ</oboInOwl:hasOBONamespace>
        <oboInOwl:id>GAZ:00080345</oboInOwl:id>
        <rdfs:label>Johi Taluka</rdfs:label>
    </owl:NamedIndividual>
    


    <!-- http://purl.obolibrary.org/obo/GAZ_00080346 -->

    <owl:NamedIndividual rdf:about="http://purl.obolibrary.org/obo/GAZ_00080346">
        <obo:RO_0001025 rdf:resource="http://purl.obolibrary.org/obo/GAZ_00018552"/>
        <obo:IAO_0000115>A Taluka of Dadu District in the Sindh province of Pakistan.</obo:IAO_0000115>
        <oboInOwl:hasOBONamespace>GAZ</oboInOwl:hasOBONamespace>
        <oboInOwl:id>GAZ:00080346</oboInOwl:id>
        <rdfs:label>Thana Bula Khan Taluka</rdfs:label>
    </owl:NamedIndividual>
    


    <!-- http://purl.obolibrary.org/obo/GAZ_00080347 -->

    <owl:NamedIndividual rdf:about="http://purl.obolibrary.org/obo/GAZ_00080347">
        <obo:RO_0001025 rdf:resource="http://purl.obolibrary.org/obo/GAZ_00400086"/>
        <obo:IAO_0000115>A Taluka in Matyari District, Sindh.</obo:IAO_0000115>
        <oboInOwl:hasOBONamespace>GAZ</oboInOwl:hasOBONamespace>
        <oboInOwl:id>GAZ:00080347</oboInOwl:id>
        <rdfs:label>Hala Taluka</rdfs:label>
    </owl:NamedIndividual>
    


    <!-- http://purl.obolibrary.org/obo/GAZ_00080348 -->

    <owl:NamedIndividual rdf:about="http://purl.obolibrary.org/obo/GAZ_00080348">
        <obo:RO_0001025 rdf:resource="http://purl.obolibrary.org/obo/GAZ_00018551"/>
        <obo:IAO_0000115>A Taluka in Noushehro Feroz District, Sindh.</obo:IAO_0000115>
        <oboInOwl:hasOBONamespace>GAZ</oboInOwl:hasOBONamespace>
        <oboInOwl:id>GAZ:00080348</oboInOwl:id>
        <rdfs:label>Moro Taluka</rdfs:label>
    </owl:NamedIndividual>
    


    <!-- http://purl.obolibrary.org/obo/GAZ_00080349 -->

    <owl:NamedIndividual rdf:about="http://purl.obolibrary.org/obo/GAZ_00080349">
        <obo:RO_0001025 rdf:resource="http://purl.obolibrary.org/obo/GAZ_00018551"/>
        <obo:IAO_0000115>A Taluka in Noushehro Feroz District, Sindh.</obo:IAO_0000115>
        <oboInOwl:hasOBONamespace>GAZ</oboInOwl:hasOBONamespace>
        <oboInOwl:id>GAZ:00080349</oboInOwl:id>
        <rdfs:label>Kandioro Taluka</rdfs:label>
    </owl:NamedIndividual>
    


    <!-- http://purl.obolibrary.org/obo/GAZ_00080350 -->

    <owl:NamedIndividual rdf:about="http://purl.obolibrary.org/obo/GAZ_00080350">
        <obo:RO_0001025 rdf:resource="http://purl.obolibrary.org/obo/GAZ_00400084"/>
        <obo:IAO_0000115>A Taluka in Tando Allah Yaar District, Sindh.</obo:IAO_0000115>
        <oboInOwl:hasOBONamespace>GAZ</oboInOwl:hasOBONamespace>
        <oboInOwl:id>GAZ:00080350</oboInOwl:id>
        <rdfs:label>Jhando Mari Taluka</rdfs:label>
    </owl:NamedIndividual>
    


    <!-- http://purl.obolibrary.org/obo/GAZ_00080351 -->

    <owl:NamedIndividual rdf:about="http://purl.obolibrary.org/obo/GAZ_00080351">
        <obo:RO_0001025 rdf:resource="http://purl.obolibrary.org/obo/GAZ_00018551"/>
        <obo:IAO_0000115>A Taluka in Noushehro Feroz District, Sindh.</obo:IAO_0000115>
        <oboInOwl:hasOBONamespace>GAZ</oboInOwl:hasOBONamespace>
        <oboInOwl:id>GAZ:00080351</oboInOwl:id>
        <rdfs:label>Bhiria Taluka</rdfs:label>
    </owl:NamedIndividual>
    


    <!-- http://purl.obolibrary.org/obo/GAZ_00080352 -->

    <owl:NamedIndividual rdf:about="http://purl.obolibrary.org/obo/GAZ_00080352">
        <obo:RO_0001025 rdf:resource="http://purl.obolibrary.org/obo/GAZ_00018551"/>
        <obo:IAO_0000115>A Taluka in Noushehro Feroz District, Sindh.</obo:IAO_0000115>
        <oboInOwl:hasOBONamespace>GAZ</oboInOwl:hasOBONamespace>
        <oboInOwl:id>GAZ:00080352</oboInOwl:id>
        <rdfs:label>Naushahro Feroze Taluka</rdfs:label>
    </owl:NamedIndividual>
    


    <!-- http://purl.obolibrary.org/obo/GAZ_00080353 -->

    <owl:NamedIndividual rdf:about="http://purl.obolibrary.org/obo/GAZ_00080353">
        <obo:RO_0001025 rdf:resource="http://purl.obolibrary.org/obo/GAZ_00018547"/>
        <obo:IAO_0000115>A Taluka of Nawabshah District, Sindh.</obo:IAO_0000115>
        <oboInOwl:hasOBONamespace>GAZ</oboInOwl:hasOBONamespace>
        <oboInOwl:id>GAZ:00080353</oboInOwl:id>
        <rdfs:label>Nawab Shah Taluka</rdfs:label>
    </owl:NamedIndividual>
    


    <!-- http://purl.obolibrary.org/obo/GAZ_00080354 -->

    <owl:NamedIndividual rdf:about="http://purl.obolibrary.org/obo/GAZ_00080354">
        <obo:RO_0001025 rdf:resource="http://purl.obolibrary.org/obo/GAZ_00018547"/>
        <obo:IAO_0000115>A Taluka of Nawabshah District, Sindh.</obo:IAO_0000115>
        <oboInOwl:hasOBONamespace>GAZ</oboInOwl:hasOBONamespace>
        <oboInOwl:id>GAZ:00080354</oboInOwl:id>
        <rdfs:label>Sakrand Taluka</rdfs:label>
    </owl:NamedIndividual>
    


    <!-- http://purl.obolibrary.org/obo/GAZ_00080355 -->

    <owl:NamedIndividual rdf:about="http://purl.obolibrary.org/obo/GAZ_00080355">
        <obo:RO_0001025 rdf:resource="http://purl.obolibrary.org/obo/GAZ_00018547"/>
        <obo:IAO_0000115>A Taluka of Nawabshah District, Sindh.</obo:IAO_0000115>
        <oboInOwl:hasOBONamespace>GAZ</oboInOwl:hasOBONamespace>
        <oboInOwl:id>GAZ:00080355</oboInOwl:id>
        <rdfs:label>Daulatpur Taluka</rdfs:label>
    </owl:NamedIndividual>
    


    <!-- http://purl.obolibrary.org/obo/GAZ_00080356 -->

    <owl:NamedIndividual rdf:about="http://purl.obolibrary.org/obo/GAZ_00080356">
        <obo:RO_0001025 rdf:resource="http://purl.obolibrary.org/obo/GAZ_00400085"/>
        <obo:IAO_0000115>A Taluka in Badin District, Sindh.</obo:IAO_0000115>
        <oboInOwl:hasOBONamespace>GAZ</oboInOwl:hasOBONamespace>
        <oboInOwl:id>GAZ:00080356</oboInOwl:id>
        <rdfs:label>Badin Taluka</rdfs:label>
    </owl:NamedIndividual>
    


    <!-- http://purl.obolibrary.org/obo/GAZ_00080357 -->

    <owl:NamedIndividual rdf:about="http://purl.obolibrary.org/obo/GAZ_00080357">
        <obo:RO_0001025 rdf:resource="http://purl.obolibrary.org/obo/GAZ_00400085"/>
        <obo:IAO_0000115>A Taluka in Badin District, Sindh.</obo:IAO_0000115>
        <oboInOwl:hasOBONamespace>GAZ</oboInOwl:hasOBONamespace>
        <oboInOwl:id>GAZ:00080357</oboInOwl:id>
        <rdfs:label>Talhar Taluka</rdfs:label>
    </owl:NamedIndividual>
    


    <!-- http://purl.obolibrary.org/obo/GAZ_00080358 -->

    <owl:NamedIndividual rdf:about="http://purl.obolibrary.org/obo/GAZ_00080358">
        <obo:RO_0001025 rdf:resource="http://purl.obolibrary.org/obo/GAZ_00400085"/>
        <obo:IAO_0000115>A Taluka in Badin District, Sindh.</obo:IAO_0000115>
        <oboInOwl:hasOBONamespace>GAZ</oboInOwl:hasOBONamespace>
        <oboInOwl:id>GAZ:00080358</oboInOwl:id>
        <rdfs:label>Tando Bago Taluka</rdfs:label>
    </owl:NamedIndividual>
    


    <!-- http://purl.obolibrary.org/obo/GAZ_00080359 -->

    <owl:NamedIndividual rdf:about="http://purl.obolibrary.org/obo/GAZ_00080359">
        <obo:RO_0001025 rdf:resource="http://purl.obolibrary.org/obo/GAZ_00400085"/>
        <obo:IAO_0000115>A Taluka in Badin District, Sindh.</obo:IAO_0000115>
        <oboInOwl:hasOBONamespace>GAZ</oboInOwl:hasOBONamespace>
        <oboInOwl:id>GAZ:00080359</oboInOwl:id>
        <rdfs:label>Shaheed Fazil Rahu Taluka</rdfs:label>
    </owl:NamedIndividual>
    


    <!-- http://purl.obolibrary.org/obo/GAZ_00080360 -->

    <owl:NamedIndividual rdf:about="http://purl.obolibrary.org/obo/GAZ_00080360">
        <obo:RO_0001025 rdf:resource="http://purl.obolibrary.org/obo/GAZ_00400085"/>
        <obo:IAO_0000115>A Taluka in Badin District, Sindh.</obo:IAO_0000115>
        <oboInOwl:hasOBONamespace>GAZ</oboInOwl:hasOBONamespace>
        <oboInOwl:id>GAZ:00080360</oboInOwl:id>
        <rdfs:label>Matli Taluka</rdfs:label>
    </owl:NamedIndividual>
    


    <!-- http://purl.obolibrary.org/obo/GAZ_00080361 -->

    <owl:NamedIndividual rdf:about="http://purl.obolibrary.org/obo/GAZ_00080361">
        <obo:RO_0001025 rdf:resource="http://purl.obolibrary.org/obo/GAZ_00400093"/>
        <obo:IAO_0000115>A city located in the Sindh province of Pakistan.</obo:IAO_0000115>
        <oboInOwl:hasOBONamespace>GAZ</oboInOwl:hasOBONamespace>
        <oboInOwl:id>GAZ:00080361</oboInOwl:id>
        <rdfs:label>City of Hyderabad</rdfs:label>
    </owl:NamedIndividual>
    


    <!-- http://purl.obolibrary.org/obo/GAZ_00080362 -->

    <owl:NamedIndividual rdf:about="http://purl.obolibrary.org/obo/GAZ_00080362">
        <obo:RO_0001025 rdf:resource="http://purl.obolibrary.org/obo/GAZ_00080361"/>
        <obo:IAO_0000115>The parts in the east of the city of Hyderabad in Sindh, Pakistan that were part of the city before the creation of Latifabad and Qasimabad. These areas include Paratabad, Islamabad, Noorani Basti, Tando Yousaf and Kalimori.</obo:IAO_0000115>
        <oboInOwl:hasOBONamespace>GAZ</oboInOwl:hasOBONamespace>
        <oboInOwl:id>GAZ:00080362</oboInOwl:id>
        <rdfs:label>Hyderabad Old City</rdfs:label>
    </owl:NamedIndividual>
    


    <!-- http://purl.obolibrary.org/obo/GAZ_00080363 -->

    <owl:NamedIndividual rdf:about="http://purl.obolibrary.org/obo/GAZ_00080363">
        <obo:RO_0001025 rdf:resource="http://purl.obolibrary.org/obo/GAZ_00080361"/>
        <obo:IAO_0000115>A neighborhood in the city of Hyderabad in Sindh, Pakistan.</obo:IAO_0000115>
        <oboInOwl:hasOBONamespace>GAZ</oboInOwl:hasOBONamespace>
        <oboInOwl:id>GAZ:00080363</oboInOwl:id>
        <rdfs:label>Hirabad</rdfs:label>
    </owl:NamedIndividual>
    


    <!-- http://purl.obolibrary.org/obo/GAZ_00080364 -->

    <owl:NamedIndividual rdf:about="http://purl.obolibrary.org/obo/GAZ_00080364">
        <obo:RO_0001025 rdf:resource="http://purl.obolibrary.org/obo/GAZ_00400093"/>
        <obo:IAO_0000115>A Taluka in Hyderabad District, Sindh.</obo:IAO_0000115>
        <oboInOwl:hasOBONamespace>GAZ</oboInOwl:hasOBONamespace>
        <oboInOwl:id>GAZ:00080364</oboInOwl:id>
        <rdfs:label>Hala Taluka</rdfs:label>
    </owl:NamedIndividual>
    


    <!-- http://purl.obolibrary.org/obo/GAZ_00080365 -->

    <owl:NamedIndividual rdf:about="http://purl.obolibrary.org/obo/GAZ_00080365">
        <obo:RO_0001025 rdf:resource="http://purl.obolibrary.org/obo/GAZ_00400087"/>
        <obo:IAO_0000115>A Taluka in Tando Muhammad Khan District, Sindh.</obo:IAO_0000115>
        <oboInOwl:hasOBONamespace>GAZ</oboInOwl:hasOBONamespace>
        <oboInOwl:id>GAZ:00080365</oboInOwl:id>
        <rdfs:label>Bulri Shah Karim Taluka</rdfs:label>
    </owl:NamedIndividual>
    


    <!-- http://purl.obolibrary.org/obo/GAZ_00080366 -->

    <owl:NamedIndividual rdf:about="http://purl.obolibrary.org/obo/GAZ_00080366">
        <obo:RO_0001025 rdf:resource="http://purl.obolibrary.org/obo/GAZ_00080361"/>
        <obo:IAO_0000115>A Taluka in Hyderabad District, Sindh.</obo:IAO_0000115>
        <oboInOwl:hasOBONamespace>GAZ</oboInOwl:hasOBONamespace>
        <oboInOwl:id>GAZ:00080366</oboInOwl:id>
        <rdfs:label>Qasimabad Taluka</rdfs:label>
    </owl:NamedIndividual>
    


    <!-- http://purl.obolibrary.org/obo/GAZ_00080367 -->

    <owl:NamedIndividual rdf:about="http://purl.obolibrary.org/obo/GAZ_00080367">
        <obo:RO_0001025 rdf:resource="http://purl.obolibrary.org/obo/GAZ_00400087"/>
        <obo:IAO_0000115>A Taluka in Tando Muhammad Khan District, Sindh.</obo:IAO_0000115>
        <oboInOwl:hasOBONamespace>GAZ</oboInOwl:hasOBONamespace>
        <oboInOwl:id>GAZ:00080367</oboInOwl:id>
        <rdfs:label>Tando Ghulam Hyder Taluka</rdfs:label>
    </owl:NamedIndividual>
    


    <!-- http://purl.obolibrary.org/obo/GAZ_00080368 -->

    <owl:NamedIndividual rdf:about="http://purl.obolibrary.org/obo/GAZ_00080368">
        <obo:RO_0001025 rdf:resource="http://purl.obolibrary.org/obo/GAZ_00080361"/>
        <obo:IAO_0000115>A Taluka in Hyderabad District, Sindh.</obo:IAO_0000115>
        <oboInOwl:hasOBONamespace>GAZ</oboInOwl:hasOBONamespace>
        <oboInOwl:id>GAZ:00080368</oboInOwl:id>
        <rdfs:label>Latifabad Taluka</rdfs:label>
    </owl:NamedIndividual>
    


    <!-- http://purl.obolibrary.org/obo/GAZ_00080369 -->

    <owl:NamedIndividual rdf:about="http://purl.obolibrary.org/obo/GAZ_00080369">
        <obo:RO_0001025 rdf:resource="http://purl.obolibrary.org/obo/GAZ_00400082"/>
        <obo:IAO_0000115>A Taluka of Sanghar District, Sindh.</obo:IAO_0000115>
        <oboInOwl:hasOBONamespace>GAZ</oboInOwl:hasOBONamespace>
        <oboInOwl:id>GAZ:00080369</oboInOwl:id>
        <rdfs:label>Khipro Taluka</rdfs:label>
    </owl:NamedIndividual>
    


    <!-- http://purl.obolibrary.org/obo/GAZ_00080370 -->

    <owl:NamedIndividual rdf:about="http://purl.obolibrary.org/obo/GAZ_00080370">
        <obo:RO_0001025 rdf:resource="http://purl.obolibrary.org/obo/GAZ_00080361"/>
        <obo:IAO_0000115>The main governing body of the city of Hyderabad in Sindh, Pakistan. It constitutes the center of the city geographically and joins all the other parts of the city.</obo:IAO_0000115>
        <oboInOwl:hasOBONamespace>GAZ</oboInOwl:hasOBONamespace>
        <oboInOwl:id>GAZ:00080370</oboInOwl:id>
        <rdfs:label>Hyderabad Central City</rdfs:label>
    </owl:NamedIndividual>
    


    <!-- http://purl.obolibrary.org/obo/GAZ_00080371 -->

    <owl:NamedIndividual rdf:about="http://purl.obolibrary.org/obo/GAZ_00080371">
        <obo:RO_0001025 rdf:resource="http://purl.obolibrary.org/obo/GAZ_00400088"/>
        <obo:IAO_0000115>A Taluka in Jamshoro District, Sindh.</obo:IAO_0000115>
        <oboInOwl:hasOBONamespace>GAZ</oboInOwl:hasOBONamespace>
        <oboInOwl:id>GAZ:00080371</oboInOwl:id>
        <rdfs:label>Kotri Taluka</rdfs:label>
    </owl:NamedIndividual>
    


    <!-- http://purl.obolibrary.org/obo/GAZ_00080372 -->

    <owl:NamedIndividual rdf:about="http://purl.obolibrary.org/obo/GAZ_00080372">
        <obo:RO_0001025 rdf:resource="http://purl.obolibrary.org/obo/GAZ_00400088"/>
        <obo:IAO_0000115>A Taluka of Jamshoro in the Sindh province of Pakistan.</obo:IAO_0000115>
        <oboInOwl:hasOBONamespace>GAZ</oboInOwl:hasOBONamespace>
        <oboInOwl:id>GAZ:00080372</oboInOwl:id>
        <rdfs:label>Thana Bulla Khan Taluka</rdfs:label>
    </owl:NamedIndividual>
    


    <!-- http://purl.obolibrary.org/obo/GAZ_00080373 -->

    <owl:NamedIndividual rdf:about="http://purl.obolibrary.org/obo/GAZ_00080373">
        <obo:RO_0001025 rdf:resource="http://purl.obolibrary.org/obo/GAZ_00400086"/>
        <obo:IAO_0000115>A Taluka in Matyari District, Sindh.</obo:IAO_0000115>
        <oboInOwl:hasOBONamespace>GAZ</oboInOwl:hasOBONamespace>
        <oboInOwl:id>GAZ:00080373</oboInOwl:id>
        <rdfs:label>Matiari Taluka</rdfs:label>
    </owl:NamedIndividual>
    


    <!-- http://purl.obolibrary.org/obo/GAZ_00080374 -->

    <owl:NamedIndividual rdf:about="http://purl.obolibrary.org/obo/GAZ_00080374">
        <obo:RO_0001025 rdf:resource="http://purl.obolibrary.org/obo/GAZ_00400086"/>
        <obo:IAO_0000115>A Taluka in Matyari District, Sindh.</obo:IAO_0000115>
        <oboInOwl:hasOBONamespace>GAZ</oboInOwl:hasOBONamespace>
        <oboInOwl:id>GAZ:00080374</oboInOwl:id>
        <rdfs:label>Saeedabad Taluka</rdfs:label>
    </owl:NamedIndividual>
    


    <!-- http://purl.obolibrary.org/obo/GAZ_00080375 -->

    <owl:NamedIndividual rdf:about="http://purl.obolibrary.org/obo/GAZ_00080375">
        <obo:RO_0001025 rdf:resource="http://purl.obolibrary.org/obo/GAZ_00400082"/>
        <obo:IAO_0000115>A Taluka of Sanghar District, Sindh.</obo:IAO_0000115>
        <oboInOwl:hasOBONamespace>GAZ</oboInOwl:hasOBONamespace>
        <oboInOwl:id>GAZ:00080375</oboInOwl:id>
        <rdfs:label>Jam Nawaz Ali Taluka</rdfs:label>
    </owl:NamedIndividual>
    


    <!-- http://purl.obolibrary.org/obo/GAZ_00080376 -->

    <owl:NamedIndividual rdf:about="http://purl.obolibrary.org/obo/GAZ_00080376">
        <obo:RO_0001025 rdf:resource="http://purl.obolibrary.org/obo/GAZ_00400082"/>
        <obo:IAO_0000115>A Taluka of Sanghar District, Sindh.</obo:IAO_0000115>
        <oboInOwl:hasOBONamespace>GAZ</oboInOwl:hasOBONamespace>
        <oboInOwl:id>GAZ:00080376</oboInOwl:id>
        <rdfs:label>Tando Adam Taluka</rdfs:label>
    </owl:NamedIndividual>
    


    <!-- http://purl.obolibrary.org/obo/GAZ_00080377 -->

    <owl:NamedIndividual rdf:about="http://purl.obolibrary.org/obo/GAZ_00080377">
        <obo:RO_0001025 rdf:resource="http://purl.obolibrary.org/obo/GAZ_00400082"/>
        <obo:IAO_0000115>A Taluka of Sanghar District, Sindh.</obo:IAO_0000115>
        <oboInOwl:hasOBONamespace>GAZ</oboInOwl:hasOBONamespace>
        <oboInOwl:id>GAZ:00080377</oboInOwl:id>
        <rdfs:label>Sanghar Taluka</rdfs:label>
    </owl:NamedIndividual>
    


    <!-- http://purl.obolibrary.org/obo/GAZ_00080378 -->

    <owl:NamedIndividual rdf:about="http://purl.obolibrary.org/obo/GAZ_00080378">
        <obo:RO_0001025 rdf:resource="http://purl.obolibrary.org/obo/GAZ_00400082"/>
        <obo:IAO_0000115>A Taluka of Sanghar District, Sindh.</obo:IAO_0000115>
        <oboInOwl:hasOBONamespace>GAZ</oboInOwl:hasOBONamespace>
        <oboInOwl:id>GAZ:00080378</oboInOwl:id>
        <rdfs:label>Sinjoro Taluka</rdfs:label>
    </owl:NamedIndividual>
    


    <!-- http://purl.obolibrary.org/obo/GAZ_00080379 -->

    <owl:NamedIndividual rdf:about="http://purl.obolibrary.org/obo/GAZ_00080379">
        <obo:RO_0001025 rdf:resource="http://purl.obolibrary.org/obo/GAZ_00400082"/>
        <obo:IAO_0000115>A Taluka of Sanghar District, Sindh.</obo:IAO_0000115>
        <oboInOwl:hasOBONamespace>GAZ</oboInOwl:hasOBONamespace>
        <oboInOwl:id>GAZ:00080379</oboInOwl:id>
        <rdfs:label>Shahdadpur Taluka</rdfs:label>
    </owl:NamedIndividual>
    


    <!-- http://purl.obolibrary.org/obo/GAZ_00080380 -->

    <owl:NamedIndividual rdf:about="http://purl.obolibrary.org/obo/GAZ_00080380">
        <obo:RO_0001025 rdf:resource="http://purl.obolibrary.org/obo/GAZ_00400084"/>
        <obo:IAO_0000115>A Taluka in Tando Allah Yaar District, Sindh.</obo:IAO_0000115>
        <oboInOwl:hasOBONamespace>GAZ</oboInOwl:hasOBONamespace>
        <oboInOwl:id>GAZ:00080380</oboInOwl:id>
        <rdfs:label>Tando Allahyar Taluka</rdfs:label>
    </owl:NamedIndividual>
    


    <!-- http://purl.obolibrary.org/obo/GAZ_00080381 -->

    <owl:NamedIndividual rdf:about="http://purl.obolibrary.org/obo/GAZ_00080381">
        <obo:RO_0001025 rdf:resource="http://purl.obolibrary.org/obo/GAZ_00400087"/>
        <obo:IAO_0000115>A Taluka in Tando Muhammad Khan District, Sindh.</obo:IAO_0000115>
        <oboInOwl:hasOBONamespace>GAZ</oboInOwl:hasOBONamespace>
        <oboInOwl:id>GAZ:00080381</oboInOwl:id>
        <rdfs:label>Tando Muhammad Khan Taluka</rdfs:label>
    </owl:NamedIndividual>
    


    <!-- http://purl.obolibrary.org/obo/GAZ_00080382 -->

    <owl:NamedIndividual rdf:about="http://purl.obolibrary.org/obo/GAZ_00080382">
        <obo:RO_0001025 rdf:resource="http://purl.obolibrary.org/obo/GAZ_00400091"/>
        <obo:IAO_0000115>A Taluka in Thatta District, Sindh.</obo:IAO_0000115>
        <oboInOwl:hasOBONamespace>GAZ</oboInOwl:hasOBONamespace>
        <oboInOwl:id>GAZ:00080382</oboInOwl:id>
        <rdfs:label>Mirpur Sakro Taluka</rdfs:label>
    </owl:NamedIndividual>
    


    <!-- http://purl.obolibrary.org/obo/GAZ_00080383 -->

    <owl:NamedIndividual rdf:about="http://purl.obolibrary.org/obo/GAZ_00080383">
        <obo:RO_0001025 rdf:resource="http://purl.obolibrary.org/obo/GAZ_00400091"/>
        <obo:IAO_0000115>A Taluka in Thatta District, Sindh.</obo:IAO_0000115>
        <oboInOwl:hasOBONamespace>GAZ</oboInOwl:hasOBONamespace>
        <oboInOwl:id>GAZ:00080383</oboInOwl:id>
        <rdfs:label>Sujawal Taluka</rdfs:label>
    </owl:NamedIndividual>
    


    <!-- http://purl.obolibrary.org/obo/GAZ_00080384 -->

    <owl:NamedIndividual rdf:about="http://purl.obolibrary.org/obo/GAZ_00080384">
        <obo:RO_0001025 rdf:resource="http://purl.obolibrary.org/obo/GAZ_00400091"/>
        <obo:IAO_0000115>A Taluka in Thatta District, Sindh.</obo:IAO_0000115>
        <oboInOwl:hasOBONamespace>GAZ</oboInOwl:hasOBONamespace>
        <oboInOwl:id>GAZ:00080384</oboInOwl:id>
        <rdfs:label>Thatta Taluka</rdfs:label>
    </owl:NamedIndividual>
    


    <!-- http://purl.obolibrary.org/obo/GAZ_00080385 -->

    <owl:NamedIndividual rdf:about="http://purl.obolibrary.org/obo/GAZ_00080385">
        <obo:RO_0001025 rdf:resource="http://purl.obolibrary.org/obo/GAZ_00400091"/>
        <obo:IAO_0000115>A Taluka in Thatta District, Sindh.</obo:IAO_0000115>
        <oboInOwl:hasOBONamespace>GAZ</oboInOwl:hasOBONamespace>
        <oboInOwl:id>GAZ:00080385</oboInOwl:id>
        <rdfs:label>Mirpur Bathoro Taluka</rdfs:label>
    </owl:NamedIndividual>
    


    <!-- http://purl.obolibrary.org/obo/GAZ_00080386 -->

    <owl:NamedIndividual rdf:about="http://purl.obolibrary.org/obo/GAZ_00080386">
        <obo:RO_0001025 rdf:resource="http://purl.obolibrary.org/obo/GAZ_00400091"/>
        <obo:IAO_0000115>A Taluka in Thatta District, Sindh.</obo:IAO_0000115>
        <oboInOwl:hasOBONamespace>GAZ</oboInOwl:hasOBONamespace>
        <oboInOwl:id>GAZ:00080386</oboInOwl:id>
        <rdfs:label>Ghora Bari Taluka</rdfs:label>
    </owl:NamedIndividual>
    


    <!-- http://purl.obolibrary.org/obo/GAZ_00080387 -->

    <owl:NamedIndividual rdf:about="http://purl.obolibrary.org/obo/GAZ_00080387">
        <obo:RO_0001025 rdf:resource="http://purl.obolibrary.org/obo/GAZ_00400091"/>
        <obo:IAO_0000115>A Taluka in Thatta District, Sindh.</obo:IAO_0000115>
        <oboInOwl:hasOBONamespace>GAZ</oboInOwl:hasOBONamespace>
        <oboInOwl:id>GAZ:00080387</oboInOwl:id>
        <rdfs:label>Shah Bander Taluka</rdfs:label>
    </owl:NamedIndividual>
    


    <!-- http://purl.obolibrary.org/obo/GAZ_00080388 -->

    <owl:NamedIndividual rdf:about="http://purl.obolibrary.org/obo/GAZ_00080388">
        <obo:RO_0001025 rdf:resource="http://purl.obolibrary.org/obo/GAZ_00400091"/>
        <obo:IAO_0000115>A Taluka in Thatta District, Sindh.</obo:IAO_0000115>
        <oboInOwl:hasOBONamespace>GAZ</oboInOwl:hasOBONamespace>
        <oboInOwl:id>GAZ:00080388</oboInOwl:id>
        <rdfs:label>Jati Taluka</rdfs:label>
    </owl:NamedIndividual>
    


    <!-- http://purl.obolibrary.org/obo/GAZ_00080389 -->

    <owl:NamedIndividual rdf:about="http://purl.obolibrary.org/obo/GAZ_00080389">
        <obo:RO_0001025 rdf:resource="http://purl.obolibrary.org/obo/GAZ_00400090"/>
        <obo:IAO_0000115>A Taluka in Mirpurkhas District, Sindh.</obo:IAO_0000115>
        <oboInOwl:hasOBONamespace>GAZ</oboInOwl:hasOBONamespace>
        <oboInOwl:id>GAZ:00080389</oboInOwl:id>
        <rdfs:label>Digri Taluka</rdfs:label>
    </owl:NamedIndividual>
    


    <!-- http://purl.obolibrary.org/obo/GAZ_00080390 -->

    <owl:NamedIndividual rdf:about="http://purl.obolibrary.org/obo/GAZ_00080390">
        <obo:RO_0001025 rdf:resource="http://purl.obolibrary.org/obo/GAZ_00400090"/>
        <obo:IAO_0000115>A Taluka in Mirpurkhas District, Sindh.</obo:IAO_0000115>
        <oboInOwl:hasOBONamespace>GAZ</oboInOwl:hasOBONamespace>
        <oboInOwl:id>GAZ:00080390</oboInOwl:id>
        <rdfs:label>Mirpur Khas Taluka</rdfs:label>
    </owl:NamedIndividual>
    


    <!-- http://purl.obolibrary.org/obo/GAZ_00080391 -->

    <owl:NamedIndividual rdf:about="http://purl.obolibrary.org/obo/GAZ_00080391">
        <obo:RO_0001025 rdf:resource="http://purl.obolibrary.org/obo/GAZ_00400090"/>
        <obo:IAO_0000115>A Taluka in Mirpurkhas District, Sindh.</obo:IAO_0000115>
        <oboInOwl:hasOBONamespace>GAZ</oboInOwl:hasOBONamespace>
        <oboInOwl:id>GAZ:00080391</oboInOwl:id>
        <rdfs:label>Kot Ghulam Mohammad Taluka</rdfs:label>
    </owl:NamedIndividual>
    


    <!-- http://purl.obolibrary.org/obo/GAZ_00080392 -->

    <owl:NamedIndividual rdf:about="http://purl.obolibrary.org/obo/GAZ_00080392">
        <obo:RO_0001025 rdf:resource="http://purl.obolibrary.org/obo/GAZ_00400089"/>
        <obo:IAO_0000115>A Taluka in Umerkot District, Sindh.</obo:IAO_0000115>
        <oboInOwl:hasOBONamespace>GAZ</oboInOwl:hasOBONamespace>
        <oboInOwl:id>GAZ:00080392</oboInOwl:id>
        <rdfs:label>Kunri Taluka</rdfs:label>
    </owl:NamedIndividual>
    


    <!-- http://purl.obolibrary.org/obo/GAZ_00080393 -->

    <owl:NamedIndividual rdf:about="http://purl.obolibrary.org/obo/GAZ_00080393">
        <obo:RO_0001025 rdf:resource="http://purl.obolibrary.org/obo/GAZ_00400089"/>
        <obo:IAO_0000115>A Taluka in Umerkot District, Sindh.</obo:IAO_0000115>
        <oboInOwl:hasOBONamespace>GAZ</oboInOwl:hasOBONamespace>
        <oboInOwl:id>GAZ:00080393</oboInOwl:id>
        <rdfs:label>Pithoro Taluka</rdfs:label>
    </owl:NamedIndividual>
    


    <!-- http://purl.obolibrary.org/obo/GAZ_00080394 -->

    <owl:NamedIndividual rdf:about="http://purl.obolibrary.org/obo/GAZ_00080394">
        <obo:RO_0001025 rdf:resource="http://purl.obolibrary.org/obo/GAZ_00400089"/>
        <obo:IAO_0000115>A Taluka in Umerkot District, Sindh.</obo:IAO_0000115>
        <oboInOwl:hasOBONamespace>GAZ</oboInOwl:hasOBONamespace>
        <oboInOwl:id>GAZ:00080394</oboInOwl:id>
        <rdfs:label>Umerkot Taluka</rdfs:label>
    </owl:NamedIndividual>
    


    <!-- http://purl.obolibrary.org/obo/GAZ_00080395 -->

    <owl:NamedIndividual rdf:about="http://purl.obolibrary.org/obo/GAZ_00080395">
        <obo:RO_0001025 rdf:resource="http://purl.obolibrary.org/obo/GAZ_00400089"/>
        <obo:IAO_0000115>A Taluka in Umerkot District, Sindh.</obo:IAO_0000115>
        <oboInOwl:hasOBONamespace>GAZ</oboInOwl:hasOBONamespace>
        <oboInOwl:id>GAZ:00080395</oboInOwl:id>
        <rdfs:label>Samaro Taluka</rdfs:label>
    </owl:NamedIndividual>
    


    <!-- http://purl.obolibrary.org/obo/GAZ_00080396 -->

    <owl:NamedIndividual rdf:about="http://purl.obolibrary.org/obo/GAZ_00080396">
        <obo:RO_0001025 rdf:resource="http://purl.obolibrary.org/obo/GAZ_00400083"/>
        <obo:IAO_0000115>A Taluka in Tharparker District, Sindh.</obo:IAO_0000115>
        <oboInOwl:hasOBONamespace>GAZ</oboInOwl:hasOBONamespace>
        <oboInOwl:id>GAZ:00080396</oboInOwl:id>
        <rdfs:label>Mithi Taluka</rdfs:label>
    </owl:NamedIndividual>
    


    <!-- http://purl.obolibrary.org/obo/GAZ_00080397 -->

    <owl:NamedIndividual rdf:about="http://purl.obolibrary.org/obo/GAZ_00080397">
        <obo:RO_0001025 rdf:resource="http://purl.obolibrary.org/obo/GAZ_00400083"/>
        <obo:IAO_0000115>A Taluka in Tharparker District, Sindh.</obo:IAO_0000115>
        <oboInOwl:hasOBONamespace>GAZ</oboInOwl:hasOBONamespace>
        <oboInOwl:id>GAZ:00080397</oboInOwl:id>
        <rdfs:label>Chachro Taluka</rdfs:label>
    </owl:NamedIndividual>
    


    <!-- http://purl.obolibrary.org/obo/GAZ_00080398 -->

    <owl:NamedIndividual rdf:about="http://purl.obolibrary.org/obo/GAZ_00080398">
        <obo:RO_0001025 rdf:resource="http://purl.obolibrary.org/obo/GAZ_00400083"/>
        <obo:IAO_0000115>A Taluka in Tharparker District, Sindh.</obo:IAO_0000115>
        <oboInOwl:hasOBONamespace>GAZ</oboInOwl:hasOBONamespace>
        <oboInOwl:id>GAZ:00080398</oboInOwl:id>
        <rdfs:label>Nagarparkar Taluka</rdfs:label>
    </owl:NamedIndividual>
    


    <!-- http://purl.obolibrary.org/obo/GAZ_00080399 -->

    <owl:NamedIndividual rdf:about="http://purl.obolibrary.org/obo/GAZ_00080399">
        <obo:RO_0001025 rdf:resource="http://purl.obolibrary.org/obo/GAZ_00400083"/>
        <obo:IAO_0000115>A Taluka in Tharparker District, Sindh.</obo:IAO_0000115>
        <oboInOwl:hasOBONamespace>GAZ</oboInOwl:hasOBONamespace>
        <oboInOwl:id>GAZ:00080399</oboInOwl:id>
        <rdfs:label>Diplo Taluka</rdfs:label>
    </owl:NamedIndividual>
    


    <!-- http://purl.obolibrary.org/obo/GAZ_00080400 -->

    <owl:NamedIndividual rdf:about="http://purl.obolibrary.org/obo/GAZ_00080400">
        <obo:RO_0001025 rdf:resource="http://purl.obolibrary.org/obo/GAZ_00400042"/>
        <obo:IAO_0000115>A Tehsil of Abbottabad District.</obo:IAO_0000115>
        <oboInOwl:hasOBONamespace>GAZ</oboInOwl:hasOBONamespace>
        <oboInOwl:id>GAZ:00080400</oboInOwl:id>
        <rdfs:label>Havelian Tehsil</rdfs:label>
    </owl:NamedIndividual>
    


    <!-- http://purl.obolibrary.org/obo/GAZ_00080401 -->

    <owl:NamedIndividual rdf:about="http://purl.obolibrary.org/obo/GAZ_00080401">
        <obo:RO_0001025 rdf:resource="http://purl.obolibrary.org/obo/GAZ_00400042"/>
        <obo:IAO_0000115>A Tehsil of Abbottabad District.</obo:IAO_0000115>
        <oboInOwl:hasOBONamespace>GAZ</oboInOwl:hasOBONamespace>
        <oboInOwl:id>GAZ:00080401</oboInOwl:id>
        <rdfs:label>Abbottabad Tehsil</rdfs:label>
    </owl:NamedIndividual>
    


    <!-- http://purl.obolibrary.org/obo/GAZ_00080402 -->

    <owl:NamedIndividual rdf:about="http://purl.obolibrary.org/obo/GAZ_00080402">
        <obo:RO_0001025 rdf:resource="http://purl.obolibrary.org/obo/GAZ_00400046"/>
        <obo:IAO_0000115>A Thesil of Bannu District.</obo:IAO_0000115>
        <oboInOwl:hasOBONamespace>GAZ</oboInOwl:hasOBONamespace>
        <oboInOwl:id>GAZ:00080402</oboInOwl:id>
        <rdfs:label>Bannu Tehsil</rdfs:label>
    </owl:NamedIndividual>
    


    <!-- http://purl.obolibrary.org/obo/GAZ_00080403 -->

    <owl:NamedIndividual rdf:about="http://purl.obolibrary.org/obo/GAZ_00080403">
        <obo:RO_0001025 rdf:resource="http://purl.obolibrary.org/obo/GAZ_00400038"/>
        <obo:IAO_0000115>A Tehsil of Batagram District in the North-West Frontier Province of Pakistan.</obo:IAO_0000115>
        <oboInOwl:hasOBONamespace>GAZ</oboInOwl:hasOBONamespace>
        <oboInOwl:id>GAZ:00080403</oboInOwl:id>
        <rdfs:label>Batagram Tehsil</rdfs:label>
    </owl:NamedIndividual>
    


    <!-- http://purl.obolibrary.org/obo/GAZ_00080404 -->

    <owl:NamedIndividual rdf:about="http://purl.obolibrary.org/obo/GAZ_00080404">
        <obo:RO_0001025 rdf:resource="http://purl.obolibrary.org/obo/GAZ_00400038"/>
        <obo:IAO_0000115>An administrative subdivision of Batagram District in the North-West Frontier Province of Pakistan. The Allai valley is bounded by Kohistan on the north and east, by the Kaghan valley, Nandhiar and Deshi of Deshiwals on the south, and by the Indus river on the west.</obo:IAO_0000115>
        <oboInOwl:hasOBONamespace>GAZ</oboInOwl:hasOBONamespace>
        <oboInOwl:id>GAZ:00080404</oboInOwl:id>
        <rdfs:label>Allai Tehsil</rdfs:label>
    </owl:NamedIndividual>
    


    <!-- http://purl.obolibrary.org/obo/GAZ_00080405 -->

    <owl:NamedIndividual rdf:about="http://purl.obolibrary.org/obo/GAZ_00080405">
        <obo:RO_0001025 rdf:resource="http://purl.obolibrary.org/obo/GAZ_00400049"/>
        <obo:IAO_0000115>A Tehsil in the Bunner District of the North-West Frontier Province.</obo:IAO_0000115>
        <oboInOwl:hasOBONamespace>GAZ</oboInOwl:hasOBONamespace>
        <oboInOwl:id>GAZ:00080405</oboInOwl:id>
        <rdfs:label>Bunner Tehsil</rdfs:label>
    </owl:NamedIndividual>
    


    <!-- http://purl.obolibrary.org/obo/GAZ_00080406 -->

    <owl:NamedIndividual rdf:about="http://purl.obolibrary.org/obo/GAZ_00080406">
        <obo:RO_0001025 rdf:resource="http://purl.obolibrary.org/obo/GAZ_00400049"/>
        <obo:IAO_0000115>A Tehsil in the Bunner District of the North-West Frontier Province.</obo:IAO_0000115>
        <oboInOwl:hasOBONamespace>GAZ</oboInOwl:hasOBONamespace>
        <oboInOwl:id>GAZ:00080406</oboInOwl:id>
        <rdfs:label>Daggar Tehsil</rdfs:label>
    </owl:NamedIndividual>
    


    <!-- http://purl.obolibrary.org/obo/GAZ_00080407 -->

    <owl:NamedIndividual rdf:about="http://purl.obolibrary.org/obo/GAZ_00080407">
        <obo:RO_0001025 rdf:resource="http://purl.obolibrary.org/obo/GAZ_00400043"/>
        <obo:IAO_0000115>A Tehsil of Charsadda District, North-West Frontier Province.</obo:IAO_0000115>
        <oboInOwl:hasOBONamespace>GAZ</oboInOwl:hasOBONamespace>
        <oboInOwl:id>GAZ:00080407</oboInOwl:id>
        <rdfs:label>Tangi Tehsil</rdfs:label>
    </owl:NamedIndividual>
    


    <!-- http://purl.obolibrary.org/obo/GAZ_00080408 -->

    <owl:NamedIndividual rdf:about="http://purl.obolibrary.org/obo/GAZ_00080408">
        <obo:RO_0001025 rdf:resource="http://purl.obolibrary.org/obo/GAZ_00400043"/>
        <obo:IAO_0000115>A Tehsil of Charsadda District, North-West Frontier Province.</obo:IAO_0000115>
        <oboInOwl:hasOBONamespace>GAZ</oboInOwl:hasOBONamespace>
        <oboInOwl:id>GAZ:00080408</oboInOwl:id>
        <rdfs:label>Charsadda Tehsil</rdfs:label>
    </owl:NamedIndividual>
    


    <!-- http://purl.obolibrary.org/obo/GAZ_00080409 -->

    <owl:NamedIndividual rdf:about="http://purl.obolibrary.org/obo/GAZ_00080409">
        <obo:RO_0001025 rdf:resource="http://purl.obolibrary.org/obo/GAZ_00400045"/>
        <obo:IAO_0000115>A Tehsil in the Chitral District of the North-West Frontier Province.</obo:IAO_0000115>
        <oboInOwl:hasOBONamespace>GAZ</oboInOwl:hasOBONamespace>
        <oboInOwl:id>GAZ:00080409</oboInOwl:id>
        <rdfs:label>Chitral Tehsil</rdfs:label>
    </owl:NamedIndividual>
    


    <!-- http://purl.obolibrary.org/obo/GAZ_00080410 -->

    <owl:NamedIndividual rdf:about="http://purl.obolibrary.org/obo/GAZ_00080410">
        <obo:RO_0001025 rdf:resource="http://purl.obolibrary.org/obo/GAZ_00400045"/>
        <obo:IAO_0000115>A Tehsil in the Chitral District of the North-West Frontier Province.</obo:IAO_0000115>
        <oboInOwl:hasOBONamespace>GAZ</oboInOwl:hasOBONamespace>
        <oboInOwl:id>GAZ:00080410</oboInOwl:id>
        <rdfs:label>Turkoh Tehsil</rdfs:label>
    </owl:NamedIndividual>
    


    <!-- http://purl.obolibrary.org/obo/GAZ_00080411 -->

    <owl:NamedIndividual rdf:about="http://purl.obolibrary.org/obo/GAZ_00080411">
        <obo:RO_0001025 rdf:resource="http://purl.obolibrary.org/obo/GAZ_00400045"/>
        <obo:IAO_0000115>A Tehsil in the Chitral District of the North-West Frontier Province.</obo:IAO_0000115>
        <oboInOwl:hasOBONamespace>GAZ</oboInOwl:hasOBONamespace>
        <oboInOwl:id>GAZ:00080411</oboInOwl:id>
        <rdfs:label>Lutkoh Tehsil</rdfs:label>
    </owl:NamedIndividual>
    


    <!-- http://purl.obolibrary.org/obo/GAZ_00080412 -->

    <owl:NamedIndividual rdf:about="http://purl.obolibrary.org/obo/GAZ_00080412">
        <obo:RO_0001025 rdf:resource="http://purl.obolibrary.org/obo/GAZ_00400045"/>
        <obo:IAO_0000115>A Tehsil in the Chitral District of the North-West Frontier Province.</obo:IAO_0000115>
        <oboInOwl:hasOBONamespace>GAZ</oboInOwl:hasOBONamespace>
        <oboInOwl:id>GAZ:00080412</oboInOwl:id>
        <rdfs:label>Mastuj Tehsil</rdfs:label>
    </owl:NamedIndividual>
    


    <!-- http://purl.obolibrary.org/obo/GAZ_00080413 -->

    <owl:NamedIndividual rdf:about="http://purl.obolibrary.org/obo/GAZ_00080413">
        <obo:RO_0001025 rdf:resource="http://purl.obolibrary.org/obo/GAZ_00400045"/>
        <obo:IAO_0000115>A Tehsil in the Chitral District of the North-West Frontier Province.</obo:IAO_0000115>
        <oboInOwl:hasOBONamespace>GAZ</oboInOwl:hasOBONamespace>
        <oboInOwl:id>GAZ:00080413</oboInOwl:id>
        <rdfs:label>Drosh Tehsil</rdfs:label>
    </owl:NamedIndividual>
    


    <!-- http://purl.obolibrary.org/obo/GAZ_00080414 -->

    <owl:NamedIndividual rdf:about="http://purl.obolibrary.org/obo/GAZ_00080414">
        <obo:RO_0001025 rdf:resource="http://purl.obolibrary.org/obo/GAZ_00400045"/>
        <obo:IAO_0000115>A Tehsil in the Chitral District of the North-West Frontier Province.</obo:IAO_0000115>
        <oboInOwl:hasOBONamespace>GAZ</oboInOwl:hasOBONamespace>
        <oboInOwl:id>GAZ:00080414</oboInOwl:id>
        <rdfs:label>Mulkoh Tehsil</rdfs:label>
    </owl:NamedIndividual>
    


    <!-- http://purl.obolibrary.org/obo/GAZ_00080415 -->

    <owl:NamedIndividual rdf:about="http://purl.obolibrary.org/obo/GAZ_00080415">
        <obo:RO_0001025 rdf:resource="http://purl.obolibrary.org/obo/GAZ_00400039"/>
        <obo:IAO_0000115>A Tehsil of Dera Ismail Khan District in North-West Frontier Province, Pakistan.</obo:IAO_0000115>
        <oboInOwl:hasOBONamespace>GAZ</oboInOwl:hasOBONamespace>
        <oboInOwl:id>GAZ:00080415</oboInOwl:id>
        <rdfs:label>Kulachi Tehsil</rdfs:label>
    </owl:NamedIndividual>
    


    <!-- http://purl.obolibrary.org/obo/GAZ_00080416 -->

    <owl:NamedIndividual rdf:about="http://purl.obolibrary.org/obo/GAZ_00080416">
        <obo:RO_0001025 rdf:resource="http://purl.obolibrary.org/obo/GAZ_00400039"/>
        <obo:IAO_0000115>A Tehsil of Dera Ismail Khan District in North-West Frontier Province, Pakistan.</obo:IAO_0000115>
        <oboInOwl:hasOBONamespace>GAZ</oboInOwl:hasOBONamespace>
        <oboInOwl:id>GAZ:00080416</oboInOwl:id>
        <rdfs:label>Paharpur Tehsil</rdfs:label>
    </owl:NamedIndividual>
    


    <!-- http://purl.obolibrary.org/obo/GAZ_00080417 -->

    <owl:NamedIndividual rdf:about="http://purl.obolibrary.org/obo/GAZ_00080417">
        <obo:RO_0001025 rdf:resource="http://purl.obolibrary.org/obo/GAZ_00400039"/>
        <obo:IAO_0000115>A Tehsil of Dera Ismail Khan District in North-West Frontier Province, Pakistan.</obo:IAO_0000115>
        <oboInOwl:hasOBONamespace>GAZ</oboInOwl:hasOBONamespace>
        <oboInOwl:id>GAZ:00080417</oboInOwl:id>
        <rdfs:label>Dera Ismail Khan Tehsil</rdfs:label>
    </owl:NamedIndividual>
    


    <!-- http://purl.obolibrary.org/obo/GAZ_00080418 -->

    <owl:NamedIndividual rdf:about="http://purl.obolibrary.org/obo/GAZ_00080418">
        <obo:RO_0001025 rdf:resource="http://purl.obolibrary.org/obo/GAZ_00400028"/>
        <obo:IAO_0000115>A Tehsil in the Dir Lower District of the North-West Frontier Province.</obo:IAO_0000115>
        <oboInOwl:hasOBONamespace>GAZ</oboInOwl:hasOBONamespace>
        <oboInOwl:id>GAZ:00080418</oboInOwl:id>
        <rdfs:label>Timargara Tehsil</rdfs:label>
    </owl:NamedIndividual>
    


    <!-- http://purl.obolibrary.org/obo/GAZ_00080419 -->

    <owl:NamedIndividual rdf:about="http://purl.obolibrary.org/obo/GAZ_00080419">
        <obo:RO_0001025 rdf:resource="http://purl.obolibrary.org/obo/GAZ_00400028"/>
        <obo:IAO_0000115>A Tehsil in the Dir Lower District of the North-West Frontier Province.</obo:IAO_0000115>
        <oboInOwl:hasOBONamespace>GAZ</oboInOwl:hasOBONamespace>
        <oboInOwl:id>GAZ:00080419</oboInOwl:id>
        <rdfs:label>Samar Bagh Tehsil</rdfs:label>
    </owl:NamedIndividual>
    


    <!-- http://purl.obolibrary.org/obo/GAZ_00080420 -->

    <owl:NamedIndividual rdf:about="http://purl.obolibrary.org/obo/GAZ_00080420">
        <obo:RO_0001025 rdf:resource="http://purl.obolibrary.org/obo/GAZ_00400030"/>
        <obo:IAO_0000115>A Tehsil in the Dir Upper District of the North-West Frontier Province.</obo:IAO_0000115>
        <oboInOwl:hasOBONamespace>GAZ</oboInOwl:hasOBONamespace>
        <oboInOwl:id>GAZ:00080420</oboInOwl:id>
        <rdfs:label>Barawal Tehsil</rdfs:label>
    </owl:NamedIndividual>
    


    <!-- http://purl.obolibrary.org/obo/GAZ_00080421 -->

    <owl:NamedIndividual rdf:about="http://purl.obolibrary.org/obo/GAZ_00080421">
        <obo:RO_0001025 rdf:resource="http://purl.obolibrary.org/obo/GAZ_00400030"/>
        <obo:IAO_0000115>A Tehsil in the Dir Upper District of the North-West Frontier Province.</obo:IAO_0000115>
        <oboInOwl:hasOBONamespace>GAZ</oboInOwl:hasOBONamespace>
        <oboInOwl:id>GAZ:00080421</oboInOwl:id>
        <rdfs:label>Dir Tehsil</rdfs:label>
    </owl:NamedIndividual>
    


    <!-- http://purl.obolibrary.org/obo/GAZ_00080422 -->

    <owl:NamedIndividual rdf:about="http://purl.obolibrary.org/obo/GAZ_00080422">
        <obo:RO_0001025 rdf:resource="http://purl.obolibrary.org/obo/GAZ_00400030"/>
        <obo:IAO_0000115>A Tehsil in the Dir Upper District of the North-West Frontier Province.</obo:IAO_0000115>
        <oboInOwl:hasOBONamespace>GAZ</oboInOwl:hasOBONamespace>
        <oboInOwl:id>GAZ:00080422</oboInOwl:id>
        <rdfs:label>Wari Tehsil</rdfs:label>
    </owl:NamedIndividual>
    


    <!-- http://purl.obolibrary.org/obo/GAZ_00080423 -->

    <owl:NamedIndividual rdf:about="http://purl.obolibrary.org/obo/GAZ_00080423">
        <obo:RO_0001025 rdf:resource="http://purl.obolibrary.org/obo/GAZ_00400030"/>
        <obo:IAO_0000115>A Tehsil in the Dir Upper District of the North-West Frontier Province.</obo:IAO_0000115>
        <oboInOwl:hasOBONamespace>GAZ</oboInOwl:hasOBONamespace>
        <oboInOwl:id>GAZ:00080423</oboInOwl:id>
        <rdfs:label>Khal Tehsil</rdfs:label>
    </owl:NamedIndividual>
    


    <!-- http://purl.obolibrary.org/obo/GAZ_00080424 -->

    <owl:NamedIndividual rdf:about="http://purl.obolibrary.org/obo/GAZ_00080424">
        <obo:RO_0001025 rdf:resource="http://purl.obolibrary.org/obo/GAZ_00400030"/>
        <obo:IAO_0000115>A Tehsil in the Dir Upper District of the North-West Frontier Province.</obo:IAO_0000115>
        <oboInOwl:hasOBONamespace>GAZ</oboInOwl:hasOBONamespace>
        <oboInOwl:id>GAZ:00080424</oboInOwl:id>
        <rdfs:label>Kalkot Tehsil</rdfs:label>
    </owl:NamedIndividual>
    


    <!-- http://purl.obolibrary.org/obo/GAZ_00080425 -->

    <owl:NamedIndividual rdf:about="http://purl.obolibrary.org/obo/GAZ_00080425">
        <obo:RO_0001025 rdf:resource="http://purl.obolibrary.org/obo/GAZ_00400030"/>
        <obo:IAO_0000115>A Tehsil in the Dir Upper District of the North-West Frontier Province.</obo:IAO_0000115>
        <oboInOwl:hasOBONamespace>GAZ</oboInOwl:hasOBONamespace>
        <oboInOwl:id>GAZ:00080425</oboInOwl:id>
        <rdfs:label>Chapar Tehsil</rdfs:label>
    </owl:NamedIndividual>
    


    <!-- http://purl.obolibrary.org/obo/GAZ_00080426 -->

    <owl:NamedIndividual rdf:about="http://purl.obolibrary.org/obo/GAZ_00080426">
        <obo:RO_0001025 rdf:resource="http://purl.obolibrary.org/obo/GAZ_00400044"/>
        <obo:IAO_0000115>A mountain ridge in the Kohat District of the North West Frontier Province of Pakistan, commanding the southern boundary of Tirah. The ridge lies between the Khanki Valley on the north and the Miranzai Valley on the south, and extends for some 30 m. west from Hangu to the Samana Suk.</obo:IAO_0000115>
        <oboInOwl:hasOBONamespace>GAZ</oboInOwl:hasOBONamespace>
        <oboInOwl:id>GAZ:00080426</oboInOwl:id>
        <rdfs:label>Samana Range</rdfs:label>
    </owl:NamedIndividual>
    


    <!-- http://purl.obolibrary.org/obo/GAZ_00080427 -->

    <owl:NamedIndividual rdf:about="http://purl.obolibrary.org/obo/GAZ_00080427">
        <obo:RO_0001025 rdf:resource="http://purl.obolibrary.org/obo/GAZ_00400047"/>
        <obo:IAO_0000115>A Tehsil in the Hangu District of the North-West Frontier Province.</obo:IAO_0000115>
        <oboInOwl:hasOBONamespace>GAZ</oboInOwl:hasOBONamespace>
        <oboInOwl:id>GAZ:00080427</oboInOwl:id>
        <rdfs:label>Hangu Tehsil</rdfs:label>
    </owl:NamedIndividual>
    


    <!-- http://purl.obolibrary.org/obo/GAZ_00080428 -->

    <owl:NamedIndividual rdf:about="http://purl.obolibrary.org/obo/GAZ_00080428">
        <obo:RO_0001025 rdf:resource="http://purl.obolibrary.org/obo/GAZ_00400041"/>
        <obo:IAO_0000115>A Tehsil in the Haripur District of the North-West Frontier Province.</obo:IAO_0000115>
        <oboInOwl:hasOBONamespace>GAZ</oboInOwl:hasOBONamespace>
        <oboInOwl:id>GAZ:00080428</oboInOwl:id>
        <rdfs:label>Ghazi Tehsil</rdfs:label>
    </owl:NamedIndividual>
    


    <!-- http://purl.obolibrary.org/obo/GAZ_00080429 -->

    <owl:NamedIndividual rdf:about="http://purl.obolibrary.org/obo/GAZ_00080429">
        <obo:RO_0001025 rdf:resource="http://purl.obolibrary.org/obo/GAZ_00400041"/>
        <obo:IAO_0000115>A Tehsil in the Haripur District of the North-West Frontier Province.</obo:IAO_0000115>
        <oboInOwl:hasOBONamespace>GAZ</oboInOwl:hasOBONamespace>
        <oboInOwl:id>GAZ:00080429</oboInOwl:id>
        <rdfs:label>Khanpur Tehsil</rdfs:label>
    </owl:NamedIndividual>
    


    <!-- http://purl.obolibrary.org/obo/GAZ_00080430 -->

    <owl:NamedIndividual rdf:about="http://purl.obolibrary.org/obo/GAZ_00080430">
        <obo:RO_0001025 rdf:resource="http://purl.obolibrary.org/obo/GAZ_00400041"/>
        <obo:IAO_0000115>A Tehsil in the Haripur District of the North-West Frontier Province.</obo:IAO_0000115>
        <oboInOwl:hasOBONamespace>GAZ</oboInOwl:hasOBONamespace>
        <oboInOwl:id>GAZ:00080430</oboInOwl:id>
        <rdfs:label>Haripur Tehsil</rdfs:label>
    </owl:NamedIndividual>
    


    <!-- http://purl.obolibrary.org/obo/GAZ_00080431 -->

    <owl:NamedIndividual rdf:about="http://purl.obolibrary.org/obo/GAZ_00080431">
        <obo:RO_0001025 rdf:resource="http://purl.obolibrary.org/obo/GAZ_00400048"/>
        <obo:IAO_0000115>A Tehsil of Karak District in the North-West Frontier Province of Pakistan.</obo:IAO_0000115>
        <oboInOwl:hasOBONamespace>GAZ</oboInOwl:hasOBONamespace>
        <oboInOwl:id>GAZ:00080431</oboInOwl:id>
        <rdfs:label>Karak Tehsil</rdfs:label>
    </owl:NamedIndividual>
    


    <!-- http://purl.obolibrary.org/obo/GAZ_00080432 -->

    <owl:NamedIndividual rdf:about="http://purl.obolibrary.org/obo/GAZ_00080432">
        <obo:RO_0001025 rdf:resource="http://purl.obolibrary.org/obo/GAZ_00400048"/>
        <obo:IAO_0000115>A Tehsil of Karak District in the North-West Frontier Province of Pakistan.</obo:IAO_0000115>
        <oboInOwl:hasOBONamespace>GAZ</oboInOwl:hasOBONamespace>
        <oboInOwl:id>GAZ:00080432</oboInOwl:id>
        <rdfs:label>Takht-e-Nasrati Tehsil</rdfs:label>
    </owl:NamedIndividual>
    


    <!-- http://purl.obolibrary.org/obo/GAZ_00080433 -->

    <owl:NamedIndividual rdf:about="http://purl.obolibrary.org/obo/GAZ_00080433">
        <obo:RO_0001025 rdf:resource="http://purl.obolibrary.org/obo/GAZ_00400048"/>
        <obo:IAO_0000115>A Tehsil of Karak District in the North-West Frontier Province of Pakistan.</obo:IAO_0000115>
        <oboInOwl:hasOBONamespace>GAZ</oboInOwl:hasOBONamespace>
        <oboInOwl:id>GAZ:00080433</oboInOwl:id>
        <rdfs:label>Banda Daud Shah Tehsil</rdfs:label>
    </owl:NamedIndividual>
    


    <!-- http://purl.obolibrary.org/obo/GAZ_00080434 -->

    <owl:NamedIndividual rdf:about="http://purl.obolibrary.org/obo/GAZ_00080434">
        <obo:RO_0001025 rdf:resource="http://purl.obolibrary.org/obo/GAZ_00400044"/>
        <obo:IAO_0000115>A Tehsil of Kohat District in the North-West Frontier Province of Pakistan.</obo:IAO_0000115>
        <oboInOwl:hasOBONamespace>GAZ</oboInOwl:hasOBONamespace>
        <oboInOwl:id>GAZ:00080434</oboInOwl:id>
        <rdfs:label>Kohat Tehsil</rdfs:label>
    </owl:NamedIndividual>
    


    <!-- http://purl.obolibrary.org/obo/GAZ_00080435 -->

    <owl:NamedIndividual rdf:about="http://purl.obolibrary.org/obo/GAZ_00080435">
        <obo:RO_0001025 rdf:resource="http://purl.obolibrary.org/obo/GAZ_00400044"/>
        <obo:IAO_0000115>A Tehsil of Kohat District in the North-West Frontier Province of Pakistan.</obo:IAO_0000115>
        <oboInOwl:hasOBONamespace>GAZ</oboInOwl:hasOBONamespace>
        <oboInOwl:id>GAZ:00080435</oboInOwl:id>
        <rdfs:label>Lachi Tehsil</rdfs:label>
    </owl:NamedIndividual>
    


    <!-- http://purl.obolibrary.org/obo/GAZ_00080436 -->

    <owl:NamedIndividual rdf:about="http://purl.obolibrary.org/obo/GAZ_00080436">
        <obo:RO_0001025 rdf:resource="http://purl.obolibrary.org/obo/GAZ_00400040"/>
        <obo:IAO_0000115>A Tehsil of Kohistan District in the North-West Frontier Province of Pakistan.</obo:IAO_0000115>
        <oboInOwl:hasOBONamespace>GAZ</oboInOwl:hasOBONamespace>
        <oboInOwl:id>GAZ:00080436</oboInOwl:id>
        <rdfs:label>Palas Tehsil</rdfs:label>
    </owl:NamedIndividual>
    


    <!-- http://purl.obolibrary.org/obo/GAZ_00080437 -->

    <owl:NamedIndividual rdf:about="http://purl.obolibrary.org/obo/GAZ_00080437">
        <obo:RO_0001025 rdf:resource="http://purl.obolibrary.org/obo/GAZ_00400040"/>
        <obo:IAO_0000115>A Tehsil of Kohistan District in the North-West Frontier Province of Pakistan.</obo:IAO_0000115>
        <oboInOwl:hasOBONamespace>GAZ</oboInOwl:hasOBONamespace>
        <oboInOwl:id>GAZ:00080437</oboInOwl:id>
        <rdfs:label>Pattan Tehsil</rdfs:label>
    </owl:NamedIndividual>
    


    <!-- http://purl.obolibrary.org/obo/GAZ_00080438 -->

    <owl:NamedIndividual rdf:about="http://purl.obolibrary.org/obo/GAZ_00080438">
        <obo:RO_0001025 rdf:resource="http://purl.obolibrary.org/obo/GAZ_00400040"/>
        <obo:IAO_0000115>A Tehsil of Kohistan District in the North-West Frontier Province of Pakistan.</obo:IAO_0000115>
        <oboInOwl:hasOBONamespace>GAZ</oboInOwl:hasOBONamespace>
        <oboInOwl:id>GAZ:00080438</oboInOwl:id>
        <rdfs:label>Dassu Tehsil</rdfs:label>
    </owl:NamedIndividual>
    


    <!-- http://purl.obolibrary.org/obo/GAZ_00080439 -->

    <owl:NamedIndividual rdf:about="http://purl.obolibrary.org/obo/GAZ_00080439">
        <obo:RO_0001025 rdf:resource="http://purl.obolibrary.org/obo/GAZ_00400037"/>
        <obo:IAO_0000115>A Tehsil of Lakki Marwat District in the North-West Frontier Province of Pakistan.</obo:IAO_0000115>
        <oboInOwl:hasOBONamespace>GAZ</oboInOwl:hasOBONamespace>
        <oboInOwl:id>GAZ:00080439</oboInOwl:id>
        <rdfs:label>Lakki Marwat Tehsil</rdfs:label>
    </owl:NamedIndividual>
    


    <!-- http://purl.obolibrary.org/obo/GAZ_00080440 -->

    <owl:NamedIndividual rdf:about="http://purl.obolibrary.org/obo/GAZ_00080440">
        <obo:RO_0001025 rdf:resource="http://purl.obolibrary.org/obo/GAZ_00400011"/>
        <obo:IAO_0000115>A Tehsil of Malakand District in the North-West Frontier Province of Pakistan.</obo:IAO_0000115>
        <oboInOwl:hasOBONamespace>GAZ</oboInOwl:hasOBONamespace>
        <oboInOwl:id>GAZ:00080440</oboInOwl:id>
        <rdfs:label>Dargai Tehsil</rdfs:label>
    </owl:NamedIndividual>
    


    <!-- http://purl.obolibrary.org/obo/GAZ_00080441 -->

    <owl:NamedIndividual rdf:about="http://purl.obolibrary.org/obo/GAZ_00080441">
        <obo:RO_0001025 rdf:resource="http://purl.obolibrary.org/obo/GAZ_00400011"/>
        <obo:IAO_0000115>A Tehsil of Malakand District in the North-West Frontier Province of Pakistan.</obo:IAO_0000115>
        <oboInOwl:hasOBONamespace>GAZ</oboInOwl:hasOBONamespace>
        <oboInOwl:id>GAZ:00080441</oboInOwl:id>
        <rdfs:label>Batkhela Tehsil</rdfs:label>
    </owl:NamedIndividual>
    


    <!-- http://purl.obolibrary.org/obo/GAZ_00080442 -->

    <owl:NamedIndividual rdf:about="http://purl.obolibrary.org/obo/GAZ_00080442">
        <obo:RO_0001025 rdf:resource="http://purl.obolibrary.org/obo/GAZ_00400027"/>
        <obo:IAO_0000115>A Tehsil of Mansehra District in the North West Frontier Province of Pakistan.</obo:IAO_0000115>
        <oboInOwl:hasOBONamespace>GAZ</oboInOwl:hasOBONamespace>
        <oboInOwl:id>GAZ:00080442</oboInOwl:id>
        <rdfs:label>Balakot Tehsil</rdfs:label>
    </owl:NamedIndividual>
    


    <!-- http://purl.obolibrary.org/obo/GAZ_00080443 -->

    <owl:NamedIndividual rdf:about="http://purl.obolibrary.org/obo/GAZ_00080443">
        <obo:RO_0001025 rdf:resource="http://purl.obolibrary.org/obo/GAZ_00400027"/>
        <obo:IAO_0000115>A tribal area of Mansehra District on the north-western Hazara border of the North-West Frontier Province of Pakistan.</obo:IAO_0000115>
        <oboInOwl:hasOBONamespace>GAZ</oboInOwl:hasOBONamespace>
        <oboInOwl:id>GAZ:00080443</oboInOwl:id>
        <rdfs:label>Kala Dhaka Provincially Administered Tribal Area</rdfs:label>
    </owl:NamedIndividual>
    


    <!-- http://purl.obolibrary.org/obo/GAZ_00080444 -->

    <owl:NamedIndividual rdf:about="http://purl.obolibrary.org/obo/GAZ_00080444">
        <obo:RO_0001025 rdf:resource="http://purl.obolibrary.org/obo/GAZ_00400027"/>
        <obo:IAO_0000115>A Tehsil of Mansehra District in the North West Frontier Province of Pakistan.</obo:IAO_0000115>
        <oboInOwl:hasOBONamespace>GAZ</oboInOwl:hasOBONamespace>
        <oboInOwl:id>GAZ:00080444</oboInOwl:id>
        <rdfs:label>Oghi Tehsil</rdfs:label>
    </owl:NamedIndividual>
    


    <!-- http://purl.obolibrary.org/obo/GAZ_00080445 -->

    <owl:NamedIndividual rdf:about="http://purl.obolibrary.org/obo/GAZ_00080445">
        <obo:RO_0001025 rdf:resource="http://purl.obolibrary.org/obo/GAZ_00400027"/>
        <obo:IAO_0000115>A Tehsil of Mansehra District in the North West Frontier Province of Pakistan.</obo:IAO_0000115>
        <oboInOwl:hasOBONamespace>GAZ</oboInOwl:hasOBONamespace>
        <oboInOwl:id>GAZ:00080445</oboInOwl:id>
        <rdfs:label>Mansehra Tehsil</rdfs:label>
    </owl:NamedIndividual>
    


    <!-- http://purl.obolibrary.org/obo/GAZ_00080446 -->

    <owl:NamedIndividual rdf:about="http://purl.obolibrary.org/obo/GAZ_00080446">
        <obo:RO_0001025 rdf:resource="http://purl.obolibrary.org/obo/GAZ_00400005"/>
        <obo:IAO_0000115>A Provincially Administered Tribal Area in Sibi District, Balochistan.</obo:IAO_0000115>
        <oboInOwl:hasOBONamespace>GAZ</oboInOwl:hasOBONamespace>
        <oboInOwl:id>GAZ:00080446</oboInOwl:id>
        <rdfs:label>Bugti Tribal Area</rdfs:label>
    </owl:NamedIndividual>
    


    <!-- http://purl.obolibrary.org/obo/GAZ_00080447 -->

    <owl:NamedIndividual rdf:about="http://purl.obolibrary.org/obo/GAZ_00080447">
        <obo:RO_0001025 rdf:resource="http://purl.obolibrary.org/obo/GAZ_00400005"/>
        <obo:IAO_0000115>A Provincially Administered Tribal Area in Sibi District, Balochistan.</obo:IAO_0000115>
        <oboInOwl:hasOBONamespace>GAZ</oboInOwl:hasOBONamespace>
        <oboInOwl:id>GAZ:00080447</oboInOwl:id>
        <rdfs:label>Marri Tribal Territory</rdfs:label>
    </owl:NamedIndividual>
    


    <!-- http://purl.obolibrary.org/obo/GAZ_00080448 -->

    <owl:NamedIndividual rdf:about="http://purl.obolibrary.org/obo/GAZ_00080448">
        <obo:RO_0001025 rdf:resource="http://purl.obolibrary.org/obo/GAZ_00400035"/>
        <obo:IAO_0000115>A Tehsil of Mardan District in the North West Frontier Province of Pakistan.</obo:IAO_0000115>
        <oboInOwl:hasOBONamespace>GAZ</oboInOwl:hasOBONamespace>
        <oboInOwl:id>GAZ:00080448</oboInOwl:id>
        <rdfs:label>Mardan Tehsil</rdfs:label>
    </owl:NamedIndividual>
    


    <!-- http://purl.obolibrary.org/obo/GAZ_00080449 -->

    <owl:NamedIndividual rdf:about="http://purl.obolibrary.org/obo/GAZ_00080449">
        <obo:RO_0001025 rdf:resource="http://purl.obolibrary.org/obo/GAZ_00400035"/>
        <obo:IAO_0000115>A Tehsil of Mardan District in the North West Frontier Province of Pakistan.</obo:IAO_0000115>
        <oboInOwl:hasOBONamespace>GAZ</oboInOwl:hasOBONamespace>
        <oboInOwl:id>GAZ:00080449</oboInOwl:id>
        <rdfs:label>Takht Bhai Tehsil</rdfs:label>
    </owl:NamedIndividual>
    


    <!-- http://purl.obolibrary.org/obo/GAZ_00080450 -->

    <owl:NamedIndividual rdf:about="http://purl.obolibrary.org/obo/GAZ_00080450">
        <obo:RO_0001025 rdf:resource="http://purl.obolibrary.org/obo/GAZ_00400036"/>
        <obo:IAO_0000115>A Tehsil of Nowshera District in the North West Frontier Province of Pakistan.</obo:IAO_0000115>
        <oboInOwl:hasOBONamespace>GAZ</oboInOwl:hasOBONamespace>
        <oboInOwl:id>GAZ:00080450</oboInOwl:id>
        <rdfs:label>Nowshera Tehsil</rdfs:label>
    </owl:NamedIndividual>
    


    <!-- http://purl.obolibrary.org/obo/GAZ_00080451 -->

    <owl:NamedIndividual rdf:about="http://purl.obolibrary.org/obo/GAZ_00080451">
        <obo:RO_0001025 rdf:resource="http://purl.obolibrary.org/obo/GAZ_00400031"/>
        <obo:IAO_0000115>A Tehsil of Peshawar District in the North West Frontier Province of Pakistan.</obo:IAO_0000115>
        <oboInOwl:hasOBONamespace>GAZ</oboInOwl:hasOBONamespace>
        <oboInOwl:id>GAZ:00080451</oboInOwl:id>
        <rdfs:label>Peshawar Tehsil</rdfs:label>
    </owl:NamedIndividual>
    


    <!-- http://purl.obolibrary.org/obo/GAZ_00080452 -->

    <owl:NamedIndividual rdf:about="http://purl.obolibrary.org/obo/GAZ_00080452">
        <obo:RO_0001025 rdf:resource="http://purl.obolibrary.org/obo/GAZ_00080451"/>
    </owl:NamedIndividual>
    


    <!-- http://purl.obolibrary.org/obo/GAZ_00080453 -->

    <owl:NamedIndividual rdf:about="http://purl.obolibrary.org/obo/GAZ_00080453">
        <obo:RO_0001025 rdf:resource="http://purl.obolibrary.org/obo/GAZ_00400029"/>
        <obo:IAO_0000115>A Tehsil of Alpuri District in the North West Frontier Province of Pakistan.</obo:IAO_0000115>
        <oboInOwl:hasOBONamespace>GAZ</oboInOwl:hasOBONamespace>
        <oboInOwl:id>GAZ:00080453</oboInOwl:id>
        <rdfs:label>Alpuri Tehsil</rdfs:label>
    </owl:NamedIndividual>
    


    <!-- http://purl.obolibrary.org/obo/GAZ_00080454 -->

    <owl:NamedIndividual rdf:about="http://purl.obolibrary.org/obo/GAZ_00080454">
        <obo:RO_0001025 rdf:resource="http://purl.obolibrary.org/obo/GAZ_00400029"/>
        <obo:IAO_0000115>A Tehsil of Alpuri District in the North West Frontier Province of Pakistan.</obo:IAO_0000115>
        <oboInOwl:hasOBONamespace>GAZ</oboInOwl:hasOBONamespace>
        <oboInOwl:id>GAZ:00080454</oboInOwl:id>
        <rdfs:label>Puran Tehsil</rdfs:label>
    </owl:NamedIndividual>
    


    <!-- http://purl.obolibrary.org/obo/GAZ_00080455 -->

    <owl:NamedIndividual rdf:about="http://purl.obolibrary.org/obo/GAZ_00080455">
        <obo:RO_0001025 rdf:resource="http://purl.obolibrary.org/obo/GAZ_00400029"/>
        <obo:IAO_0000115>A Sub-Tehsil of Alpuri District in the North West Frontier Province of Pakistan.</obo:IAO_0000115>
        <oboInOwl:hasOBONamespace>GAZ</oboInOwl:hasOBONamespace>
        <oboInOwl:id>GAZ:00080455</oboInOwl:id>
        <rdfs:label>Martung Sub-Tehsil</rdfs:label>
    </owl:NamedIndividual>
    


    <!-- http://purl.obolibrary.org/obo/GAZ_00080456 -->

    <owl:NamedIndividual rdf:about="http://purl.obolibrary.org/obo/GAZ_00080456">
        <obo:RO_0001025 rdf:resource="http://purl.obolibrary.org/obo/GAZ_00400029"/>
        <obo:IAO_0000115>A Sub-Tehsil of Alpuri District in the North West Frontier Province of Pakistan.</obo:IAO_0000115>
        <oboInOwl:hasOBONamespace>GAZ</oboInOwl:hasOBONamespace>
        <oboInOwl:id>GAZ:00080456</oboInOwl:id>
        <rdfs:label>Besham Sub-Tehsil</rdfs:label>
    </owl:NamedIndividual>
    


    <!-- http://purl.obolibrary.org/obo/GAZ_00080457 -->

    <owl:NamedIndividual rdf:about="http://purl.obolibrary.org/obo/GAZ_00080457">
        <obo:RO_0001025 rdf:resource="http://purl.obolibrary.org/obo/GAZ_00400029"/>
        <obo:IAO_0000115>A Sub-Tehsil of Alpuri District in the North West Frontier Province of Pakistan.</obo:IAO_0000115>
        <oboInOwl:hasOBONamespace>GAZ</oboInOwl:hasOBONamespace>
        <oboInOwl:id>GAZ:00080457</oboInOwl:id>
        <rdfs:label>Chakesar Sub-Tehsil</rdfs:label>
    </owl:NamedIndividual>
    


    <!-- http://purl.obolibrary.org/obo/GAZ_00080458 -->

    <owl:NamedIndividual rdf:about="http://purl.obolibrary.org/obo/GAZ_00080458">
        <obo:RO_0001025 rdf:resource="http://purl.obolibrary.org/obo/GAZ_00400033"/>
        <obo:IAO_0000115>A Tehsil of Swabi District in the North-West Frontier Province of Pakistan.</obo:IAO_0000115>
        <oboInOwl:hasOBONamespace>GAZ</oboInOwl:hasOBONamespace>
        <oboInOwl:id>GAZ:00080458</oboInOwl:id>
        <rdfs:label>Lahor Tehsil</rdfs:label>
    </owl:NamedIndividual>
    


    <!-- http://purl.obolibrary.org/obo/GAZ_00080459 -->

    <owl:NamedIndividual rdf:about="http://purl.obolibrary.org/obo/GAZ_00080459">
        <obo:RO_0001025 rdf:resource="http://purl.obolibrary.org/obo/GAZ_00400033"/>
        <obo:IAO_0000115>A Tehsil of Swabi District in the North-West Frontier Province of Pakistan.</obo:IAO_0000115>
        <oboInOwl:hasOBONamespace>GAZ</oboInOwl:hasOBONamespace>
        <oboInOwl:id>GAZ:00080459</oboInOwl:id>
        <rdfs:label>Swabi Tehsil</rdfs:label>
    </owl:NamedIndividual>
    


    <!-- http://purl.obolibrary.org/obo/GAZ_00080460 -->

    <owl:NamedIndividual rdf:about="http://purl.obolibrary.org/obo/GAZ_00080460">
        <obo:RO_0001025 rdf:resource="http://purl.obolibrary.org/obo/GAZ_00400033"/>
        <obo:IAO_0000115>A Tehsil of Swabi District in the North-West Frontier Province of Pakistan.</obo:IAO_0000115>
        <oboInOwl:hasOBONamespace>GAZ</oboInOwl:hasOBONamespace>
        <oboInOwl:id>GAZ:00080460</oboInOwl:id>
        <rdfs:label>Topi Tehsil</rdfs:label>
    </owl:NamedIndividual>
    


    <!-- http://purl.obolibrary.org/obo/GAZ_00080461 -->

    <owl:NamedIndividual rdf:about="http://purl.obolibrary.org/obo/GAZ_00080461">
        <obo:RO_0001025 rdf:resource="http://purl.obolibrary.org/obo/GAZ_00400032"/>
        <obo:IAO_0000115>A Tehsil of Swat District in the North-West Frontier Province of Pakistan.</obo:IAO_0000115>
        <oboInOwl:hasOBONamespace>GAZ</oboInOwl:hasOBONamespace>
        <oboInOwl:id>GAZ:00080461</oboInOwl:id>
        <rdfs:label>Matta Tehsil</rdfs:label>
    </owl:NamedIndividual>
    


    <!-- http://purl.obolibrary.org/obo/GAZ_00080462 -->

    <owl:NamedIndividual rdf:about="http://purl.obolibrary.org/obo/GAZ_00080462">
        <obo:RO_0001025 rdf:resource="http://purl.obolibrary.org/obo/GAZ_00400032"/>
        <obo:IAO_0000115>A Tehsil of Swat District in the North-West Frontier Province of Pakistan.</obo:IAO_0000115>
        <oboInOwl:hasOBONamespace>GAZ</oboInOwl:hasOBONamespace>
        <oboInOwl:id>GAZ:00080462</oboInOwl:id>
        <rdfs:label>Swat Tehsil</rdfs:label>
    </owl:NamedIndividual>
    


    <!-- http://purl.obolibrary.org/obo/GAZ_00080463 -->

    <owl:NamedIndividual rdf:about="http://purl.obolibrary.org/obo/GAZ_00080463">
        <obo:RO_0001025 rdf:resource="http://purl.obolibrary.org/obo/GAZ_00400034"/>
        <obo:IAO_0000115>A Tehsil of Tank District in the North-West Frontier Province of Pakistan.</obo:IAO_0000115>
        <oboInOwl:hasOBONamespace>GAZ</oboInOwl:hasOBONamespace>
        <oboInOwl:id>GAZ:00080463</oboInOwl:id>
        <rdfs:label>Tank Tehsil</rdfs:label>
    </owl:NamedIndividual>
    


    <!-- http://purl.obolibrary.org/obo/GAZ_00080464 -->

    <owl:NamedIndividual rdf:about="http://purl.obolibrary.org/obo/GAZ_00080464">
        <obo:RO_0001025 rdf:resource="http://purl.obolibrary.org/obo/GAZ_00400080"/>
        <obo:IAO_0000115>One of the six Tehsils of Attock District in the Punjab province of Pakistan.</obo:IAO_0000115>
        <oboInOwl:hasOBONamespace>GAZ</oboInOwl:hasOBONamespace>
        <oboInOwl:id>GAZ:00080464</oboInOwl:id>
        <rdfs:label>Attock Tehsil</rdfs:label>
    </owl:NamedIndividual>
    


    <!-- http://purl.obolibrary.org/obo/GAZ_00080465 -->

    <owl:NamedIndividual rdf:about="http://purl.obolibrary.org/obo/GAZ_00080465">
        <obo:RO_0001025 rdf:resource="http://purl.obolibrary.org/obo/GAZ_00400080"/>
        <obo:IAO_0000115>One of the six Tehsils of Attock District in the Punjab province of Pakistan.</obo:IAO_0000115>
        <oboInOwl:hasOBONamespace>GAZ</oboInOwl:hasOBONamespace>
        <oboInOwl:id>GAZ:00080465</oboInOwl:id>
        <rdfs:label>Hassan Abdal Tehsil</rdfs:label>
    </owl:NamedIndividual>
    


    <!-- http://purl.obolibrary.org/obo/GAZ_00080466 -->

    <owl:NamedIndividual rdf:about="http://purl.obolibrary.org/obo/GAZ_00080466">
        <obo:RO_0001025 rdf:resource="http://purl.obolibrary.org/obo/GAZ_00400080"/>
        <obo:IAO_0000115>One of the six Tehsils of Attock District in the Punjab province of Pakistan.</obo:IAO_0000115>
        <oboInOwl:hasOBONamespace>GAZ</oboInOwl:hasOBONamespace>
        <oboInOwl:id>GAZ:00080466</oboInOwl:id>
        <rdfs:label>Hazro Tehsil</rdfs:label>
    </owl:NamedIndividual>
    


    <!-- http://purl.obolibrary.org/obo/GAZ_00080467 -->

    <owl:NamedIndividual rdf:about="http://purl.obolibrary.org/obo/GAZ_00080467">
        <obo:RO_0001025 rdf:resource="http://purl.obolibrary.org/obo/GAZ_00400080"/>
        <obo:IAO_0000115>One of the six Tehsils of Attock District in the Punjab province of Pakistan.</obo:IAO_0000115>
        <oboInOwl:hasOBONamespace>GAZ</oboInOwl:hasOBONamespace>
        <oboInOwl:id>GAZ:00080467</oboInOwl:id>
        <rdfs:label>Jand Tehsil</rdfs:label>
    </owl:NamedIndividual>
    


    <!-- http://purl.obolibrary.org/obo/GAZ_00080468 -->

    <owl:NamedIndividual rdf:about="http://purl.obolibrary.org/obo/GAZ_00080468">
        <obo:RO_0001025 rdf:resource="http://purl.obolibrary.org/obo/GAZ_00400080"/>
        <obo:IAO_0000115>One of the six Tehsils of Attock District in the Punjab province of Pakistan.</obo:IAO_0000115>
        <oboInOwl:hasOBONamespace>GAZ</oboInOwl:hasOBONamespace>
        <oboInOwl:id>GAZ:00080468</oboInOwl:id>
        <rdfs:label>Fateh Jang Tehsil</rdfs:label>
    </owl:NamedIndividual>
    


    <!-- http://purl.obolibrary.org/obo/GAZ_00080469 -->

    <owl:NamedIndividual rdf:about="http://purl.obolibrary.org/obo/GAZ_00080469">
        <obo:RO_0001025 rdf:resource="http://purl.obolibrary.org/obo/GAZ_00400080"/>
        <obo:IAO_0000115>One of the six Tehsils of Attock District in the Punjab province of Pakistan.</obo:IAO_0000115>
        <oboInOwl:hasOBONamespace>GAZ</oboInOwl:hasOBONamespace>
        <oboInOwl:id>GAZ:00080469</oboInOwl:id>
        <rdfs:label>Pindi Gheb Tehsil</rdfs:label>
    </owl:NamedIndividual>
    


    <!-- http://purl.obolibrary.org/obo/GAZ_00080470 -->

    <owl:NamedIndividual rdf:about="http://purl.obolibrary.org/obo/GAZ_00080470">
        <obo:RO_0001025 rdf:resource="http://purl.obolibrary.org/obo/GAZ_00400076"/>
        <obo:IAO_0000115>A Tehsil in Bahawalnagar District, Punjab.</obo:IAO_0000115>
        <oboInOwl:hasOBONamespace>GAZ</oboInOwl:hasOBONamespace>
        <oboInOwl:id>GAZ:00080470</oboInOwl:id>
        <rdfs:label>Bahawalnagar Tehsil</rdfs:label>
    </owl:NamedIndividual>
    


    <!-- http://purl.obolibrary.org/obo/GAZ_00080471 -->

    <owl:NamedIndividual rdf:about="http://purl.obolibrary.org/obo/GAZ_00080471">
        <obo:RO_0001025 rdf:resource="http://purl.obolibrary.org/obo/GAZ_00400076"/>
        <obo:IAO_0000115>A Tehsil in Bahawalnagar District, Punjab.</obo:IAO_0000115>
        <oboInOwl:hasOBONamespace>GAZ</oboInOwl:hasOBONamespace>
        <oboInOwl:id>GAZ:00080471</oboInOwl:id>
        <rdfs:label>Chishtian Tehsil</rdfs:label>
    </owl:NamedIndividual>
    


    <!-- http://purl.obolibrary.org/obo/GAZ_00080472 -->

    <owl:NamedIndividual rdf:about="http://purl.obolibrary.org/obo/GAZ_00080472">
        <obo:RO_0001025 rdf:resource="http://purl.obolibrary.org/obo/GAZ_00400076"/>
        <obo:IAO_0000115>A Tehsil in Bahawalnagar District, Punjab.</obo:IAO_0000115>
        <oboInOwl:hasOBONamespace>GAZ</oboInOwl:hasOBONamespace>
        <oboInOwl:id>GAZ:00080472</oboInOwl:id>
        <rdfs:label>Fort Abbas Tehsil</rdfs:label>
    </owl:NamedIndividual>
    


    <!-- http://purl.obolibrary.org/obo/GAZ_00080473 -->

    <owl:NamedIndividual rdf:about="http://purl.obolibrary.org/obo/GAZ_00080473">
        <obo:RO_0001025 rdf:resource="http://purl.obolibrary.org/obo/GAZ_00400076"/>
        <obo:IAO_0000115>A Tehsil in Bahawalnagar District, Punjab.</obo:IAO_0000115>
        <oboInOwl:hasOBONamespace>GAZ</oboInOwl:hasOBONamespace>
        <oboInOwl:id>GAZ:00080473</oboInOwl:id>
        <rdfs:label>Minchanabad Tehsil</rdfs:label>
    </owl:NamedIndividual>
    


    <!-- http://purl.obolibrary.org/obo/GAZ_00080474 -->

    <owl:NamedIndividual rdf:about="http://purl.obolibrary.org/obo/GAZ_00080474">
        <obo:RO_0001025 rdf:resource="http://purl.obolibrary.org/obo/GAZ_00400076"/>
        <obo:IAO_0000115>A Tehsil in Bahawalnagar District, Punjab.</obo:IAO_0000115>
        <oboInOwl:hasOBONamespace>GAZ</oboInOwl:hasOBONamespace>
        <oboInOwl:id>GAZ:00080474</oboInOwl:id>
        <rdfs:label>Haroonabad Tehsil</rdfs:label>
    </owl:NamedIndividual>
    


    <!-- http://purl.obolibrary.org/obo/GAZ_00080475 -->

    <owl:NamedIndividual rdf:about="http://purl.obolibrary.org/obo/GAZ_00080475">
        <obo:RO_0001025 rdf:resource="http://purl.obolibrary.org/obo/GAZ_00400077"/>
        <obo:IAO_0000115>A Tehsil of Bahawalpur District in the Punjab province of Pakistan.</obo:IAO_0000115>
        <oboInOwl:hasOBONamespace>GAZ</oboInOwl:hasOBONamespace>
        <oboInOwl:id>GAZ:00080475</oboInOwl:id>
        <rdfs:label>Bahawalpur Tehsil</rdfs:label>
    </owl:NamedIndividual>
    


    <!-- http://purl.obolibrary.org/obo/GAZ_00080476 -->

    <owl:NamedIndividual rdf:about="http://purl.obolibrary.org/obo/GAZ_00080476">
        <obo:RO_0001025 rdf:resource="http://purl.obolibrary.org/obo/GAZ_00400077"/>
        <obo:IAO_0000115>A Tehsil of Bahawalpur District in the Punjab province of Pakistan.</obo:IAO_0000115>
        <oboInOwl:hasOBONamespace>GAZ</oboInOwl:hasOBONamespace>
        <oboInOwl:id>GAZ:00080476</oboInOwl:id>
        <rdfs:label>Ahmedpur Sharqia Tehsil</rdfs:label>
    </owl:NamedIndividual>
    


    <!-- http://purl.obolibrary.org/obo/GAZ_00080477 -->

    <owl:NamedIndividual rdf:about="http://purl.obolibrary.org/obo/GAZ_00080477">
        <obo:RO_0001025 rdf:resource="http://purl.obolibrary.org/obo/GAZ_00400077"/>
        <obo:IAO_0000115>A Tehsil of Bahawalpur District in the Punjab province of Pakistan.</obo:IAO_0000115>
        <oboInOwl:hasOBONamespace>GAZ</oboInOwl:hasOBONamespace>
        <oboInOwl:id>GAZ:00080477</oboInOwl:id>
        <rdfs:label>Khairpur Tamewali Tehsil</rdfs:label>
    </owl:NamedIndividual>
    


    <!-- http://purl.obolibrary.org/obo/GAZ_00080478 -->

    <owl:NamedIndividual rdf:about="http://purl.obolibrary.org/obo/GAZ_00080478">
        <obo:RO_0001025 rdf:resource="http://purl.obolibrary.org/obo/GAZ_00400077"/>
        <obo:IAO_0000115>A Tehsil of Bahawalpur District in the Punjab province of Pakistan.</obo:IAO_0000115>
        <oboInOwl:hasOBONamespace>GAZ</oboInOwl:hasOBONamespace>
        <oboInOwl:id>GAZ:00080478</oboInOwl:id>
        <rdfs:label>Hasilpur Tehsil</rdfs:label>
    </owl:NamedIndividual>
    


    <!-- http://purl.obolibrary.org/obo/GAZ_00080479 -->

    <owl:NamedIndividual rdf:about="http://purl.obolibrary.org/obo/GAZ_00080479">
        <obo:RO_0001025 rdf:resource="http://purl.obolibrary.org/obo/GAZ_00400077"/>
        <obo:IAO_0000115>A Tehsil of Bahawalpur District in the Punjab province of Pakistan.</obo:IAO_0000115>
        <oboInOwl:hasOBONamespace>GAZ</oboInOwl:hasOBONamespace>
        <oboInOwl:id>GAZ:00080479</oboInOwl:id>
        <rdfs:label>Yazman Mandi Tehsil</rdfs:label>
    </owl:NamedIndividual>
    


    <!-- http://purl.obolibrary.org/obo/GAZ_00080480 -->

    <owl:NamedIndividual rdf:about="http://purl.obolibrary.org/obo/GAZ_00080480">
        <obo:RO_0001025 rdf:resource="http://purl.obolibrary.org/obo/GAZ_00400074"/>
        <obo:IAO_0000115>A Tehsil of Bhakkar District in the Punjab province of Pakistan.</obo:IAO_0000115>
        <oboInOwl:hasOBONamespace>GAZ</oboInOwl:hasOBONamespace>
        <oboInOwl:id>GAZ:00080480</oboInOwl:id>
        <rdfs:label>Darya Khan Tehsil</rdfs:label>
    </owl:NamedIndividual>
    


    <!-- http://purl.obolibrary.org/obo/GAZ_00080481 -->

    <owl:NamedIndividual rdf:about="http://purl.obolibrary.org/obo/GAZ_00080481">
        <obo:RO_0001025 rdf:resource="http://purl.obolibrary.org/obo/GAZ_00400074"/>
        <obo:IAO_0000115>A Tehsil of Bhakkar District in the Punjab province of Pakistan.</obo:IAO_0000115>
        <oboInOwl:hasOBONamespace>GAZ</oboInOwl:hasOBONamespace>
        <oboInOwl:id>GAZ:00080481</oboInOwl:id>
        <rdfs:label>Kaloorkot Tehsil</rdfs:label>
    </owl:NamedIndividual>
    


    <!-- http://purl.obolibrary.org/obo/GAZ_00080482 -->

    <owl:NamedIndividual rdf:about="http://purl.obolibrary.org/obo/GAZ_00080482">
        <obo:RO_0001025 rdf:resource="http://purl.obolibrary.org/obo/GAZ_00400074"/>
        <obo:IAO_0000115>A Tehsil of Bhakkar District in the Punjab province of Pakistan.</obo:IAO_0000115>
        <oboInOwl:hasOBONamespace>GAZ</oboInOwl:hasOBONamespace>
        <oboInOwl:id>GAZ:00080482</oboInOwl:id>
        <rdfs:label>Mankera Tehsil</rdfs:label>
    </owl:NamedIndividual>
    


    <!-- http://purl.obolibrary.org/obo/GAZ_00080483 -->

    <owl:NamedIndividual rdf:about="http://purl.obolibrary.org/obo/GAZ_00080483">
        <obo:RO_0001025 rdf:resource="http://purl.obolibrary.org/obo/GAZ_00400074"/>
        <obo:IAO_0000115>A Tehsil of Bhakkar District in the Punjab province of Pakistan.</obo:IAO_0000115>
        <oboInOwl:hasOBONamespace>GAZ</oboInOwl:hasOBONamespace>
        <oboInOwl:id>GAZ:00080483</oboInOwl:id>
        <rdfs:label>Bhakkar Tehsil</rdfs:label>
    </owl:NamedIndividual>
    


    <!-- http://purl.obolibrary.org/obo/GAZ_00080484 -->

    <owl:NamedIndividual rdf:about="http://purl.obolibrary.org/obo/GAZ_00080484">
        <obo:RO_0001025 rdf:resource="http://purl.obolibrary.org/obo/GAZ_00400081"/>
        <obo:IAO_0000115>A Tehsil of Chakwal District, Punjab.</obo:IAO_0000115>
        <oboInOwl:hasOBONamespace>GAZ</oboInOwl:hasOBONamespace>
        <oboInOwl:id>GAZ:00080484</oboInOwl:id>
        <rdfs:label>Talagang Tehsil</rdfs:label>
    </owl:NamedIndividual>
    


    <!-- http://purl.obolibrary.org/obo/GAZ_00080485 -->

    <owl:NamedIndividual rdf:about="http://purl.obolibrary.org/obo/GAZ_00080485">
        <obo:RO_0001025 rdf:resource="http://purl.obolibrary.org/obo/GAZ_00400081"/>
        <obo:IAO_0000115>A Tehsil of Chakwal District, Punjab.</obo:IAO_0000115>
        <oboInOwl:hasOBONamespace>GAZ</oboInOwl:hasOBONamespace>
        <oboInOwl:id>GAZ:00080485</oboInOwl:id>
        <rdfs:label>Chakwal Tehsil</rdfs:label>
    </owl:NamedIndividual>
    


    <!-- http://purl.obolibrary.org/obo/GAZ_00080486 -->

    <owl:NamedIndividual rdf:about="http://purl.obolibrary.org/obo/GAZ_00080486">
        <obo:RO_0001025 rdf:resource="http://purl.obolibrary.org/obo/GAZ_00400081"/>
        <obo:IAO_0000115>A Tehsil of Chakwal District, Punjab.</obo:IAO_0000115>
        <oboInOwl:hasOBONamespace>GAZ</oboInOwl:hasOBONamespace>
        <oboInOwl:id>GAZ:00080486</oboInOwl:id>
        <rdfs:label>Choa Saidan Shah Tehsil</rdfs:label>
    </owl:NamedIndividual>
    


    <!-- http://purl.obolibrary.org/obo/GAZ_00080487 -->

    <owl:NamedIndividual rdf:about="http://purl.obolibrary.org/obo/GAZ_00080487">
        <obo:RO_0001025 rdf:resource="http://purl.obolibrary.org/obo/GAZ_00005260"/>
        <obo:IAO_0000115>A lake in the Changa Manga Forest.</obo:IAO_0000115>
        <oboInOwl:hasOBONamespace>GAZ</oboInOwl:hasOBONamespace>
        <oboInOwl:id>GAZ:00080487</oboInOwl:id>
        <rdfs:label>Lunar Lake</rdfs:label>
    </owl:NamedIndividual>
    


    <!-- http://purl.obolibrary.org/obo/GAZ_00080488 -->

    <owl:NamedIndividual rdf:about="http://purl.obolibrary.org/obo/GAZ_00080488">
        <obo:RO_0001025 rdf:resource="http://purl.obolibrary.org/obo/GAZ_00400070"/>
        <obo:IAO_0000115>A Tehsil in Kasur District, Punjab.</obo:IAO_0000115>
        <oboInOwl:hasOBONamespace>GAZ</oboInOwl:hasOBONamespace>
        <oboInOwl:id>GAZ:00080488</oboInOwl:id>
        <rdfs:label>Chunian Tehsil</rdfs:label>
    </owl:NamedIndividual>
    


    <!-- http://purl.obolibrary.org/obo/GAZ_00080489 -->

    <owl:NamedIndividual rdf:about="http://purl.obolibrary.org/obo/GAZ_00080489">
        <obo:RO_0001025 rdf:resource="http://purl.obolibrary.org/obo/GAZ_00007534"/>
        <obo:IAO_0000115>A Tehsil of Dera Ghazi Khan District in the Punjab province of Pakistan.</obo:IAO_0000115>
        <oboInOwl:hasOBONamespace>GAZ</oboInOwl:hasOBONamespace>
        <oboInOwl:id>GAZ:00080489</oboInOwl:id>
        <rdfs:label>De-Ex.Area of D.G.Khan</rdfs:label>
    </owl:NamedIndividual>
    


    <!-- http://purl.obolibrary.org/obo/GAZ_00080490 -->

    <owl:NamedIndividual rdf:about="http://purl.obolibrary.org/obo/GAZ_00080490">
        <obo:RO_0001025 rdf:resource="http://purl.obolibrary.org/obo/GAZ_00007534"/>
        <obo:IAO_0000115>A Tehsil of Dera Ghazi Khan District in the Punjab province of Pakistan.</obo:IAO_0000115>
        <oboInOwl:hasOBONamespace>GAZ</oboInOwl:hasOBONamespace>
        <oboInOwl:id>GAZ:00080490</oboInOwl:id>
        <rdfs:label>Dera Ghazi Khan Tehsil</rdfs:label>
    </owl:NamedIndividual>
    


    <!-- http://purl.obolibrary.org/obo/GAZ_00080491 -->

    <owl:NamedIndividual rdf:about="http://purl.obolibrary.org/obo/GAZ_00080491">
        <obo:RO_0001025 rdf:resource="http://purl.obolibrary.org/obo/GAZ_00007534"/>
        <obo:IAO_0000115>A Tehsil of Dera Ghazi Khan District in the Punjab province of Pakistan.</obo:IAO_0000115>
        <oboInOwl:hasOBONamespace>GAZ</oboInOwl:hasOBONamespace>
        <oboInOwl:id>GAZ:00080491</oboInOwl:id>
        <rdfs:label>Taunsa Sharif Tehsil</rdfs:label>
    </owl:NamedIndividual>
    


    <!-- http://purl.obolibrary.org/obo/GAZ_00080492 -->

    <owl:NamedIndividual rdf:about="http://purl.obolibrary.org/obo/GAZ_00080492">
        <obo:RO_0001025 rdf:resource="http://purl.obolibrary.org/obo/GAZ_00400078"/>
        <obo:IAO_0000115>A Tehsil of Faisalabad in the Punjab province of Pakistan.</obo:IAO_0000115>
        <oboInOwl:hasOBONamespace>GAZ</oboInOwl:hasOBONamespace>
        <oboInOwl:id>GAZ:00080492</oboInOwl:id>
        <rdfs:label>Sammundri Tehsil</rdfs:label>
    </owl:NamedIndividual>
    


    <!-- http://purl.obolibrary.org/obo/GAZ_00080493 -->

    <owl:NamedIndividual rdf:about="http://purl.obolibrary.org/obo/GAZ_00080493">
        <obo:RO_0001025 rdf:resource="http://purl.obolibrary.org/obo/GAZ_00400078"/>
        <obo:IAO_0000115>A Tehsil of Faisalabad in the Punjab province of Pakistan.</obo:IAO_0000115>
        <oboInOwl:hasOBONamespace>GAZ</oboInOwl:hasOBONamespace>
        <oboInOwl:id>GAZ:00080493</oboInOwl:id>
        <rdfs:label>Chak Jhumra Tehsil</rdfs:label>
    </owl:NamedIndividual>
    


    <!-- http://purl.obolibrary.org/obo/GAZ_00080494 -->

    <owl:NamedIndividual rdf:about="http://purl.obolibrary.org/obo/GAZ_00080494">
        <obo:RO_0001025 rdf:resource="http://purl.obolibrary.org/obo/GAZ_00400078"/>
        <obo:IAO_0000115>A Tehsil of Faisalabad in the Punjab province of Pakistan.</obo:IAO_0000115>
        <oboInOwl:hasOBONamespace>GAZ</oboInOwl:hasOBONamespace>
        <oboInOwl:id>GAZ:00080494</oboInOwl:id>
        <rdfs:label>Jaranwala Tehsil</rdfs:label>
    </owl:NamedIndividual>
    


    <!-- http://purl.obolibrary.org/obo/GAZ_00080495 -->

    <owl:NamedIndividual rdf:about="http://purl.obolibrary.org/obo/GAZ_00080495">
        <obo:RO_0001025 rdf:resource="http://purl.obolibrary.org/obo/GAZ_00400078"/>
        <obo:IAO_0000115>A Tehsil of Faisalabad in the Punjab province of Pakistan.</obo:IAO_0000115>
        <oboInOwl:hasOBONamespace>GAZ</oboInOwl:hasOBONamespace>
        <oboInOwl:id>GAZ:00080495</oboInOwl:id>
        <rdfs:label>Faisalabad Saddar Tehsil</rdfs:label>
    </owl:NamedIndividual>
    


    <!-- http://purl.obolibrary.org/obo/GAZ_00080496 -->

    <owl:NamedIndividual rdf:about="http://purl.obolibrary.org/obo/GAZ_00080496">
        <obo:RO_0001025 rdf:resource="http://purl.obolibrary.org/obo/GAZ_00400078"/>
        <obo:IAO_0000115>A Tehsil of Faisalabad in the Punjab province of Pakistan.</obo:IAO_0000115>
        <oboInOwl:hasOBONamespace>GAZ</oboInOwl:hasOBONamespace>
        <oboInOwl:id>GAZ:00080496</oboInOwl:id>
        <rdfs:label>Tandlianwala Tehsil</rdfs:label>
    </owl:NamedIndividual>
    


    <!-- http://purl.obolibrary.org/obo/GAZ_00080497 -->

    <owl:NamedIndividual rdf:about="http://purl.obolibrary.org/obo/GAZ_00080497">
        <obo:RO_0001025 rdf:resource="http://purl.obolibrary.org/obo/GAZ_00400078"/>
        <obo:IAO_0000115>A city located in Punjab, Pakistan. The city-district of Faisalabad is bound on the north by the districts of Gujranwala and Sheikhupura, on the east by Sahiwal, on the south by Toba Tek Singh and on the west by Jhang.</obo:IAO_0000115>
        <oboInOwl:hasOBONamespace>GAZ</oboInOwl:hasOBONamespace>
        <oboInOwl:id>GAZ:00080497</oboInOwl:id>
        <rdfs:label>Faisalabad City</rdfs:label>
    </owl:NamedIndividual>
    


    <!-- http://purl.obolibrary.org/obo/GAZ_00080498 -->

    <owl:NamedIndividual rdf:about="http://purl.obolibrary.org/obo/GAZ_00080498">
        <obo:RO_0001025 rdf:resource="http://purl.obolibrary.org/obo/GAZ_00400072"/>
        <obo:IAO_0000115>A Tehsil of Gujranwala District, Punjab.</obo:IAO_0000115>
        <oboInOwl:hasOBONamespace>GAZ</oboInOwl:hasOBONamespace>
        <oboInOwl:id>GAZ:00080498</oboInOwl:id>
        <rdfs:label>Nowshera Virkan Tehsil</rdfs:label>
    </owl:NamedIndividual>
    


    <!-- http://purl.obolibrary.org/obo/GAZ_00080499 -->

    <owl:NamedIndividual rdf:about="http://purl.obolibrary.org/obo/GAZ_00080499">
        <obo:RO_0001025 rdf:resource="http://purl.obolibrary.org/obo/GAZ_00400072"/>
        <obo:IAO_0000115>A Tehsil of Gujranwala District, Punjab.</obo:IAO_0000115>
        <oboInOwl:hasOBONamespace>GAZ</oboInOwl:hasOBONamespace>
        <oboInOwl:id>GAZ:00080499</oboInOwl:id>
        <rdfs:label>Kamoki Tehsil</rdfs:label>
    </owl:NamedIndividual>
    


    <!-- http://purl.obolibrary.org/obo/GAZ_00080500 -->

    <owl:NamedIndividual rdf:about="http://purl.obolibrary.org/obo/GAZ_00080500">
        <obo:RO_0001025 rdf:resource="http://purl.obolibrary.org/obo/GAZ_00400072"/>
        <obo:IAO_0000115>A Tehsil of Gujranwala District, Punjab.</obo:IAO_0000115>
        <oboInOwl:hasOBONamespace>GAZ</oboInOwl:hasOBONamespace>
        <oboInOwl:id>GAZ:00080500</oboInOwl:id>
        <rdfs:label>Wazirabad Tehsil</rdfs:label>
    </owl:NamedIndividual>
    


    <!-- http://purl.obolibrary.org/obo/GAZ_00080501 -->

    <owl:NamedIndividual rdf:about="http://purl.obolibrary.org/obo/GAZ_00080501">
        <obo:RO_0001025 rdf:resource="http://purl.obolibrary.org/obo/GAZ_00400072"/>
        <obo:IAO_0000115>A populated place. A city in Punjab, Pakistan.</obo:IAO_0000115>
        <oboInOwl:hasOBONamespace>GAZ</oboInOwl:hasOBONamespace>
        <oboInOwl:id>GAZ:00080501</oboInOwl:id>
        <rdfs:label>Gujranwala City</rdfs:label>
    </owl:NamedIndividual>
    


    <!-- http://purl.obolibrary.org/obo/GAZ_00080502 -->

    <owl:NamedIndividual rdf:about="http://purl.obolibrary.org/obo/GAZ_00080502">
        <obo:RO_0001025 rdf:resource="http://purl.obolibrary.org/obo/GAZ_00400071"/>
        <obo:IAO_0000115>A Tehsil of Gujrat District in the Punjab province of Pakistan.</obo:IAO_0000115>
        <oboInOwl:hasOBONamespace>GAZ</oboInOwl:hasOBONamespace>
        <oboInOwl:id>GAZ:00080502</oboInOwl:id>
        <rdfs:label>Gujrat Tehsil</rdfs:label>
    </owl:NamedIndividual>
    


    <!-- http://purl.obolibrary.org/obo/GAZ_00080503 -->

    <owl:NamedIndividual rdf:about="http://purl.obolibrary.org/obo/GAZ_00080503">
        <obo:RO_0001025 rdf:resource="http://purl.obolibrary.org/obo/GAZ_00400071"/>
        <obo:IAO_0000115>A Tehsil of Gujrat District in the Punjab province of Pakistan.</obo:IAO_0000115>
        <oboInOwl:hasOBONamespace>GAZ</oboInOwl:hasOBONamespace>
        <oboInOwl:id>GAZ:00080503</oboInOwl:id>
        <rdfs:label>Kharian Tehsil</rdfs:label>
    </owl:NamedIndividual>
    


    <!-- http://purl.obolibrary.org/obo/GAZ_00080504 -->

    <owl:NamedIndividual rdf:about="http://purl.obolibrary.org/obo/GAZ_00080504">
        <obo:RO_0001025 rdf:resource="http://purl.obolibrary.org/obo/GAZ_00400071"/>
        <obo:IAO_0000115>A Tehsil of Gujrat District in the Punjab province of Pakistan.</obo:IAO_0000115>
        <oboInOwl:hasOBONamespace>GAZ</oboInOwl:hasOBONamespace>
        <oboInOwl:id>GAZ:00080504</oboInOwl:id>
        <rdfs:label>Sarai Alamgir Tehsil</rdfs:label>
    </owl:NamedIndividual>
    


    <!-- http://purl.obolibrary.org/obo/GAZ_00080505 -->

    <owl:NamedIndividual rdf:about="http://purl.obolibrary.org/obo/GAZ_00080505">
        <obo:RO_0001025 rdf:resource="http://purl.obolibrary.org/obo/GAZ_00400075"/>
        <obo:IAO_0000115>A Tehsil of Hafizabad District in the Punjab province of Pakistan.</obo:IAO_0000115>
        <oboInOwl:hasOBONamespace>GAZ</oboInOwl:hasOBONamespace>
        <oboInOwl:id>GAZ:00080505</oboInOwl:id>
        <rdfs:label>Hafizabad Tehsil</rdfs:label>
    </owl:NamedIndividual>
    


    <!-- http://purl.obolibrary.org/obo/GAZ_00080506 -->

    <owl:NamedIndividual rdf:about="http://purl.obolibrary.org/obo/GAZ_00080506">
        <obo:RO_0001025 rdf:resource="http://purl.obolibrary.org/obo/GAZ_00400075"/>
        <obo:IAO_0000115>A Tehsil of Hafizabad District in the Punjab province of Pakistan.</obo:IAO_0000115>
        <oboInOwl:hasOBONamespace>GAZ</oboInOwl:hasOBONamespace>
        <oboInOwl:id>GAZ:00080506</oboInOwl:id>
        <rdfs:label>Pindi Bhattian Tehsil</rdfs:label>
    </owl:NamedIndividual>
    


    <!-- http://purl.obolibrary.org/obo/GAZ_00080507 -->

    <owl:NamedIndividual rdf:about="http://purl.obolibrary.org/obo/GAZ_00080507">
        <obo:RO_0001025 rdf:resource="http://purl.obolibrary.org/obo/GAZ_00400079"/>
        <obo:IAO_0000115>A Tehsil of Jhang District in the Punjab province of Pakistan.</obo:IAO_0000115>
        <oboInOwl:hasOBONamespace>GAZ</oboInOwl:hasOBONamespace>
        <oboInOwl:id>GAZ:00080507</oboInOwl:id>
        <rdfs:label>Jhang Tehsil</rdfs:label>
    </owl:NamedIndividual>
    


    <!-- http://purl.obolibrary.org/obo/GAZ_00080508 -->

    <owl:NamedIndividual rdf:about="http://purl.obolibrary.org/obo/GAZ_00080508">
        <obo:RO_0001025 rdf:resource="http://purl.obolibrary.org/obo/GAZ_00400079"/>
        <obo:IAO_0000115>A Tehsil of Jhang District in the Punjab province of Pakistan.</obo:IAO_0000115>
        <oboInOwl:hasOBONamespace>GAZ</oboInOwl:hasOBONamespace>
        <oboInOwl:id>GAZ:00080508</oboInOwl:id>
        <rdfs:label>Ahmed Pur Sial Tehsil</rdfs:label>
    </owl:NamedIndividual>
    


    <!-- http://purl.obolibrary.org/obo/GAZ_00080509 -->

    <owl:NamedIndividual rdf:about="http://purl.obolibrary.org/obo/GAZ_00080509">
        <obo:RO_0001025 rdf:resource="http://purl.obolibrary.org/obo/GAZ_00400079"/>
        <obo:IAO_0000115>A Tehsil of Jhang District in the Punjab province of Pakistan.</obo:IAO_0000115>
        <oboInOwl:hasOBONamespace>GAZ</oboInOwl:hasOBONamespace>
        <oboInOwl:id>GAZ:00080509</oboInOwl:id>
        <rdfs:label>Chiniot Tehsil</rdfs:label>
    </owl:NamedIndividual>
    


    <!-- http://purl.obolibrary.org/obo/GAZ_00080510 -->

    <owl:NamedIndividual rdf:about="http://purl.obolibrary.org/obo/GAZ_00080510">
        <obo:RO_0001025 rdf:resource="http://purl.obolibrary.org/obo/GAZ_00400079"/>
        <obo:IAO_0000115>A Tehsil of Jhang District in the Punjab province of Pakistan.</obo:IAO_0000115>
        <oboInOwl:hasOBONamespace>GAZ</oboInOwl:hasOBONamespace>
        <oboInOwl:id>GAZ:00080510</oboInOwl:id>
        <rdfs:label>Shorkot Tehsil</rdfs:label>
    </owl:NamedIndividual>
    


    <!-- http://purl.obolibrary.org/obo/GAZ_00080511 -->

    <owl:NamedIndividual rdf:about="http://purl.obolibrary.org/obo/GAZ_00080511">
        <obo:RO_0001025 rdf:resource="http://purl.obolibrary.org/obo/GAZ_00400073"/>
        <obo:IAO_0000115>A Tehsil in Jhelum District, Punjab.</obo:IAO_0000115>
        <oboInOwl:hasOBONamespace>GAZ</oboInOwl:hasOBONamespace>
        <oboInOwl:id>GAZ:00080511</oboInOwl:id>
        <rdfs:label>Pind Dadan Khan Tehsil</rdfs:label>
    </owl:NamedIndividual>
    


    <!-- http://purl.obolibrary.org/obo/GAZ_00080512 -->

    <owl:NamedIndividual rdf:about="http://purl.obolibrary.org/obo/GAZ_00080512">
        <obo:RO_0001025 rdf:resource="http://purl.obolibrary.org/obo/GAZ_00400073"/>
        <obo:IAO_0000115>A Tehsil in Jhelum District, Punjab.</obo:IAO_0000115>
        <oboInOwl:hasOBONamespace>GAZ</oboInOwl:hasOBONamespace>
        <oboInOwl:id>GAZ:00080512</oboInOwl:id>
        <rdfs:label>Dina Tehsil</rdfs:label>
    </owl:NamedIndividual>
    


    <!-- http://purl.obolibrary.org/obo/GAZ_00080513 -->

    <owl:NamedIndividual rdf:about="http://purl.obolibrary.org/obo/GAZ_00080513">
        <obo:RO_0001025 rdf:resource="http://purl.obolibrary.org/obo/GAZ_00400073"/>
        <obo:IAO_0000115>A Tehsil in Jhelum District, Punjab.</obo:IAO_0000115>
        <oboInOwl:hasOBONamespace>GAZ</oboInOwl:hasOBONamespace>
        <oboInOwl:id>GAZ:00080513</oboInOwl:id>
        <rdfs:label>Sohawa Tehsil</rdfs:label>
    </owl:NamedIndividual>
    


    <!-- http://purl.obolibrary.org/obo/GAZ_00080514 -->

    <owl:NamedIndividual rdf:about="http://purl.obolibrary.org/obo/GAZ_00080514">
        <obo:RO_0001025 rdf:resource="http://purl.obolibrary.org/obo/GAZ_00400073"/>
        <obo:IAO_0000115>A Tehsil in Jhelum District, Punjab.</obo:IAO_0000115>
        <oboInOwl:hasOBONamespace>GAZ</oboInOwl:hasOBONamespace>
        <oboInOwl:id>GAZ:00080514</oboInOwl:id>
        <rdfs:label>Jhelum Tehsil</rdfs:label>
    </owl:NamedIndividual>
    


    <!-- http://purl.obolibrary.org/obo/GAZ_00080515 -->

    <owl:NamedIndividual rdf:about="http://purl.obolibrary.org/obo/GAZ_00080515">
        <obo:RO_0001025 rdf:resource="http://purl.obolibrary.org/obo/GAZ_00400070"/>
        <obo:IAO_0000115>A Tehsil in Kasur District, Punjab.</obo:IAO_0000115>
        <oboInOwl:hasOBONamespace>GAZ</oboInOwl:hasOBONamespace>
        <oboInOwl:id>GAZ:00080515</oboInOwl:id>
        <rdfs:label>Pattoki Tehsil</rdfs:label>
    </owl:NamedIndividual>
    


    <!-- http://purl.obolibrary.org/obo/GAZ_00080516 -->

    <owl:NamedIndividual rdf:about="http://purl.obolibrary.org/obo/GAZ_00080516">
        <obo:RO_0001025 rdf:resource="http://purl.obolibrary.org/obo/GAZ_00400070"/>
        <obo:IAO_0000115>A Tehsil in Kasur District, Punjab.</obo:IAO_0000115>
        <oboInOwl:hasOBONamespace>GAZ</oboInOwl:hasOBONamespace>
        <oboInOwl:id>GAZ:00080516</oboInOwl:id>
        <rdfs:label>Kasur Tehsil</rdfs:label>
    </owl:NamedIndividual>
    


    <!-- http://purl.obolibrary.org/obo/GAZ_00080517 -->

    <owl:NamedIndividual rdf:about="http://purl.obolibrary.org/obo/GAZ_00080517">
        <obo:RO_0001025 rdf:resource="http://purl.obolibrary.org/obo/GAZ_00400067"/>
        <obo:IAO_0000115>A Tehsil in Khanewal District, Punjab.</obo:IAO_0000115>
        <oboInOwl:hasOBONamespace>GAZ</oboInOwl:hasOBONamespace>
        <oboInOwl:id>GAZ:00080517</oboInOwl:id>
        <rdfs:label>Kabirwala Tehsil</rdfs:label>
    </owl:NamedIndividual>
    


    <!-- http://purl.obolibrary.org/obo/GAZ_00080518 -->

    <owl:NamedIndividual rdf:about="http://purl.obolibrary.org/obo/GAZ_00080518">
        <obo:RO_0001025 rdf:resource="http://purl.obolibrary.org/obo/GAZ_00400067"/>
        <obo:IAO_0000115>A Tehsil in Khanewal District, Punjab.</obo:IAO_0000115>
        <oboInOwl:hasOBONamespace>GAZ</oboInOwl:hasOBONamespace>
        <oboInOwl:id>GAZ:00080518</oboInOwl:id>
        <rdfs:label>Khanewal Tehsil</rdfs:label>
    </owl:NamedIndividual>
    


    <!-- http://purl.obolibrary.org/obo/GAZ_00080519 -->

    <owl:NamedIndividual rdf:about="http://purl.obolibrary.org/obo/GAZ_00080519">
        <obo:RO_0001025 rdf:resource="http://purl.obolibrary.org/obo/GAZ_00400067"/>
        <obo:IAO_0000115>A Tehsil in Khanewal District, Punjab.</obo:IAO_0000115>
        <oboInOwl:hasOBONamespace>GAZ</oboInOwl:hasOBONamespace>
        <oboInOwl:id>GAZ:00080519</oboInOwl:id>
        <rdfs:label>Mian Channu Tehsil</rdfs:label>
    </owl:NamedIndividual>
    


    <!-- http://purl.obolibrary.org/obo/GAZ_00080520 -->

    <owl:NamedIndividual rdf:about="http://purl.obolibrary.org/obo/GAZ_00080520">
        <obo:RO_0001025 rdf:resource="http://purl.obolibrary.org/obo/GAZ_00400067"/>
        <obo:IAO_0000115>A Tehsil in Khanewal District, Punjab.</obo:IAO_0000115>
        <oboInOwl:hasOBONamespace>GAZ</oboInOwl:hasOBONamespace>
        <oboInOwl:id>GAZ:00080520</oboInOwl:id>
        <rdfs:label>Jahanian Tehsil</rdfs:label>
    </owl:NamedIndividual>
    


    <!-- http://purl.obolibrary.org/obo/GAZ_00080521 -->

    <owl:NamedIndividual rdf:about="http://purl.obolibrary.org/obo/GAZ_00080521">
        <obo:RO_0001025 rdf:resource="http://purl.obolibrary.org/obo/GAZ_00400068"/>
        <obo:IAO_0000115>A Tehsil in Khushab District, Punjab.</obo:IAO_0000115>
        <oboInOwl:hasOBONamespace>GAZ</oboInOwl:hasOBONamespace>
        <oboInOwl:id>GAZ:00080521</oboInOwl:id>
        <rdfs:label>Nurpur Tehsil</rdfs:label>
    </owl:NamedIndividual>
    


    <!-- http://purl.obolibrary.org/obo/GAZ_00080522 -->

    <owl:NamedIndividual rdf:about="http://purl.obolibrary.org/obo/GAZ_00080522">
        <obo:RO_0001025 rdf:resource="http://purl.obolibrary.org/obo/GAZ_00400068"/>
        <obo:IAO_0000115>A Sub-Tehsil in Khushab District, Punjab.</obo:IAO_0000115>
        <oboInOwl:hasOBONamespace>GAZ</oboInOwl:hasOBONamespace>
        <oboInOwl:id>GAZ:00080522</oboInOwl:id>
        <rdfs:label>Noshehra Sub-Tehsil</rdfs:label>
    </owl:NamedIndividual>
    


    <!-- http://purl.obolibrary.org/obo/GAZ_00080523 -->

    <owl:NamedIndividual rdf:about="http://purl.obolibrary.org/obo/GAZ_00080523">
        <obo:RO_0001025 rdf:resource="http://purl.obolibrary.org/obo/GAZ_00400068"/>
        <obo:IAO_0000115>A Tehsil in Khushab District, Punjab.</obo:IAO_0000115>
        <oboInOwl:hasOBONamespace>GAZ</oboInOwl:hasOBONamespace>
        <oboInOwl:id>GAZ:00080523</oboInOwl:id>
        <rdfs:label>Quaidabad Tehsil</rdfs:label>
    </owl:NamedIndividual>
    


    <!-- http://purl.obolibrary.org/obo/GAZ_00080524 -->

    <owl:NamedIndividual rdf:about="http://purl.obolibrary.org/obo/GAZ_00080524">
        <obo:RO_0001025 rdf:resource="http://purl.obolibrary.org/obo/GAZ_00400068"/>
        <obo:IAO_0000115>A Tehsil in Khushab District, Punjab.</obo:IAO_0000115>
        <oboInOwl:hasOBONamespace>GAZ</oboInOwl:hasOBONamespace>
        <oboInOwl:id>GAZ:00080524</oboInOwl:id>
        <rdfs:label>Khushab Tehsil</rdfs:label>
    </owl:NamedIndividual>
    


    <!-- http://purl.obolibrary.org/obo/GAZ_00080525 -->

    <owl:NamedIndividual rdf:about="http://purl.obolibrary.org/obo/GAZ_00080525">
        <obo:RO_0001025 rdf:resource="http://purl.obolibrary.org/obo/GAZ_00005259"/>
        <obo:IAO_0000115>A Tehsil of Lahore District, Punjab.</obo:IAO_0000115>
        <oboInOwl:hasOBONamespace>GAZ</oboInOwl:hasOBONamespace>
        <oboInOwl:id>GAZ:00080525</oboInOwl:id>
        <rdfs:label>Lahore Urban City</rdfs:label>
    </owl:NamedIndividual>
    


    <!-- http://purl.obolibrary.org/obo/GAZ_00080526 -->

    <owl:NamedIndividual rdf:about="http://purl.obolibrary.org/obo/GAZ_00080526">
        <obo:RO_0001025 rdf:resource="http://purl.obolibrary.org/obo/GAZ_00005259"/>
        <obo:IAO_0000115>A Tehsil of Lahore District, Punjab.</obo:IAO_0000115>
        <oboInOwl:hasOBONamespace>GAZ</oboInOwl:hasOBONamespace>
        <oboInOwl:id>GAZ:00080526</oboInOwl:id>
        <rdfs:label>Lahore City Centre</rdfs:label>
    </owl:NamedIndividual>
    


    <!-- http://purl.obolibrary.org/obo/GAZ_00080527 -->

    <owl:NamedIndividual rdf:about="http://purl.obolibrary.org/obo/GAZ_00080527">
        <obo:RO_0001025 rdf:resource="http://purl.obolibrary.org/obo/GAZ_00005259"/>
        <obo:IAO_0000115>A Tehsil of Lahore District, Punjab.</obo:IAO_0000115>
        <oboInOwl:hasOBONamespace>GAZ</oboInOwl:hasOBONamespace>
        <oboInOwl:id>GAZ:00080527</oboInOwl:id>
        <rdfs:label>Lahore Rural Tehsil</rdfs:label>
    </owl:NamedIndividual>
    


    <!-- http://purl.obolibrary.org/obo/GAZ_00080528 -->

    <owl:NamedIndividual rdf:about="http://purl.obolibrary.org/obo/GAZ_00080528">
        <obo:RO_0001025 rdf:resource="http://purl.obolibrary.org/obo/GAZ_00400069"/>
        <obo:IAO_0000115>A Sub-Tehsil in Layyah District, Punjab.</obo:IAO_0000115>
        <oboInOwl:hasOBONamespace>GAZ</oboInOwl:hasOBONamespace>
        <oboInOwl:id>GAZ:00080528</oboInOwl:id>
        <rdfs:label>Chowk Azam Sub-Tehsil</rdfs:label>
    </owl:NamedIndividual>
    


    <!-- http://purl.obolibrary.org/obo/GAZ_00080529 -->

    <owl:NamedIndividual rdf:about="http://purl.obolibrary.org/obo/GAZ_00080529">
        <obo:RO_0001025 rdf:resource="http://purl.obolibrary.org/obo/GAZ_00400069"/>
        <obo:IAO_0000115>A Sub-Tehsil in Layyah District, Punjab.</obo:IAO_0000115>
        <oboInOwl:hasOBONamespace>GAZ</oboInOwl:hasOBONamespace>
        <oboInOwl:id>GAZ:00080529</oboInOwl:id>
        <rdfs:label>Fatehpur Sub-Tehsil</rdfs:label>
    </owl:NamedIndividual>
    


    <!-- http://purl.obolibrary.org/obo/GAZ_00080530 -->

    <owl:NamedIndividual rdf:about="http://purl.obolibrary.org/obo/GAZ_00080530">
        <obo:RO_0001025 rdf:resource="http://purl.obolibrary.org/obo/GAZ_00400069"/>
        <obo:IAO_0000115>A Tehsil in Layyah District, Punjab.</obo:IAO_0000115>
        <oboInOwl:hasOBONamespace>GAZ</oboInOwl:hasOBONamespace>
        <oboInOwl:id>GAZ:00080530</oboInOwl:id>
        <rdfs:label>Karor Lal Esan Tehsil</rdfs:label>
    </owl:NamedIndividual>
    


    <!-- http://purl.obolibrary.org/obo/GAZ_00080531 -->

    <owl:NamedIndividual rdf:about="http://purl.obolibrary.org/obo/GAZ_00080531">
        <obo:RO_0001025 rdf:resource="http://purl.obolibrary.org/obo/GAZ_00400069"/>
        <obo:IAO_0000115>A Tehsil in Layyah District, Punjab.</obo:IAO_0000115>
        <oboInOwl:hasOBONamespace>GAZ</oboInOwl:hasOBONamespace>
        <oboInOwl:id>GAZ:00080531</oboInOwl:id>
        <rdfs:label>Chaubara Tehsil</rdfs:label>
    </owl:NamedIndividual>
    


    <!-- http://purl.obolibrary.org/obo/GAZ_00080532 -->

    <owl:NamedIndividual rdf:about="http://purl.obolibrary.org/obo/GAZ_00080532">
        <obo:RO_0001025 rdf:resource="http://purl.obolibrary.org/obo/GAZ_00400069"/>
        <obo:IAO_0000115>A Tehsil in Layyah District, Punjab.</obo:IAO_0000115>
        <oboInOwl:hasOBONamespace>GAZ</oboInOwl:hasOBONamespace>
        <oboInOwl:id>GAZ:00080532</oboInOwl:id>
        <rdfs:label>Layyah Tehsil</rdfs:label>
    </owl:NamedIndividual>
    


    <!-- http://purl.obolibrary.org/obo/GAZ_00080533 -->

    <owl:NamedIndividual rdf:about="http://purl.obolibrary.org/obo/GAZ_00080533">
        <obo:RO_0001025 rdf:resource="http://purl.obolibrary.org/obo/GAZ_00400065"/>
        <obo:IAO_0000115>A Tehsil in Lodhran District, Punjab.</obo:IAO_0000115>
        <oboInOwl:hasOBONamespace>GAZ</oboInOwl:hasOBONamespace>
        <oboInOwl:id>GAZ:00080533</oboInOwl:id>
        <rdfs:label>Lodhran Tehsil</rdfs:label>
    </owl:NamedIndividual>
    


    <!-- http://purl.obolibrary.org/obo/GAZ_00080534 -->

    <owl:NamedIndividual rdf:about="http://purl.obolibrary.org/obo/GAZ_00080534">
        <obo:RO_0001025 rdf:resource="http://purl.obolibrary.org/obo/GAZ_00400065"/>
        <obo:IAO_0000115>A Tehsil in Lodhran District, Punjab.</obo:IAO_0000115>
        <oboInOwl:hasOBONamespace>GAZ</oboInOwl:hasOBONamespace>
        <oboInOwl:id>GAZ:00080534</oboInOwl:id>
        <rdfs:label>Kahror Pacca Tehsil</rdfs:label>
    </owl:NamedIndividual>
    


    <!-- http://purl.obolibrary.org/obo/GAZ_00080535 -->

    <owl:NamedIndividual rdf:about="http://purl.obolibrary.org/obo/GAZ_00080535">
        <obo:RO_0001025 rdf:resource="http://purl.obolibrary.org/obo/GAZ_00400065"/>
        <obo:IAO_0000115>A Tehsil in Lodhran District, Punjab.</obo:IAO_0000115>
        <oboInOwl:hasOBONamespace>GAZ</oboInOwl:hasOBONamespace>
        <oboInOwl:id>GAZ:00080535</oboInOwl:id>
        <rdfs:label>Dunya Pur Tehsil</rdfs:label>
    </owl:NamedIndividual>
    


    <!-- http://purl.obolibrary.org/obo/GAZ_00080536 -->

    <owl:NamedIndividual rdf:about="http://purl.obolibrary.org/obo/GAZ_00080536">
        <obo:RO_0001025 rdf:resource="http://purl.obolibrary.org/obo/GAZ_00400066"/>
        <obo:IAO_0000115>A Tehsil of Mandi Bahauddin District, Punjab.</obo:IAO_0000115>
        <oboInOwl:hasOBONamespace>GAZ</oboInOwl:hasOBONamespace>
        <oboInOwl:id>GAZ:00080536</oboInOwl:id>
        <rdfs:label>Phalia Tehsil</rdfs:label>
    </owl:NamedIndividual>
    


    <!-- http://purl.obolibrary.org/obo/GAZ_00080537 -->

    <owl:NamedIndividual rdf:about="http://purl.obolibrary.org/obo/GAZ_00080537">
        <obo:RO_0001025 rdf:resource="http://purl.obolibrary.org/obo/GAZ_00400066"/>
        <obo:IAO_0000115>A Tehsil of Mandi Bahauddin District, Punjab.</obo:IAO_0000115>
        <oboInOwl:hasOBONamespace>GAZ</oboInOwl:hasOBONamespace>
        <oboInOwl:id>GAZ:00080537</oboInOwl:id>
        <rdfs:label>Mandi Bahauddin Tehsil</rdfs:label>
    </owl:NamedIndividual>
    


    <!-- http://purl.obolibrary.org/obo/GAZ_00080538 -->

    <owl:NamedIndividual rdf:about="http://purl.obolibrary.org/obo/GAZ_00080538">
        <obo:RO_0001025 rdf:resource="http://purl.obolibrary.org/obo/GAZ_00400066"/>
        <obo:IAO_0000115>A Tehsil of Mandi Bahauddin District, Punjab.</obo:IAO_0000115>
        <oboInOwl:hasOBONamespace>GAZ</oboInOwl:hasOBONamespace>
        <oboInOwl:id>GAZ:00080538</oboInOwl:id>
        <rdfs:label>Malakwal Tehsil</rdfs:label>
    </owl:NamedIndividual>
    


    <!-- http://purl.obolibrary.org/obo/GAZ_00080539 -->

    <owl:NamedIndividual rdf:about="http://purl.obolibrary.org/obo/GAZ_00080539">
        <obo:RO_0001025 rdf:resource="http://purl.obolibrary.org/obo/GAZ_00400056"/>
        <obo:IAO_0000115>A Tehsil in Mianwali District, Punjab.</obo:IAO_0000115>
        <oboInOwl:hasOBONamespace>GAZ</oboInOwl:hasOBONamespace>
        <oboInOwl:id>GAZ:00080539</oboInOwl:id>
        <rdfs:label>Isakhel Tehsil</rdfs:label>
    </owl:NamedIndividual>
    


    <!-- http://purl.obolibrary.org/obo/GAZ_00080540 -->

    <owl:NamedIndividual rdf:about="http://purl.obolibrary.org/obo/GAZ_00080540">
        <obo:RO_0001025 rdf:resource="http://purl.obolibrary.org/obo/GAZ_00400056"/>
        <obo:IAO_0000115>A Tehsil of Mianwali District, situated in southern Punjab, Pakistan.</obo:IAO_0000115>
        <oboInOwl:hasOBONamespace>GAZ</oboInOwl:hasOBONamespace>
        <oboInOwl:id>GAZ:00080540</oboInOwl:id>
        <rdfs:label>Piplan Tehsil</rdfs:label>
    </owl:NamedIndividual>
    


    <!-- http://purl.obolibrary.org/obo/GAZ_00080541 -->

    <owl:NamedIndividual rdf:about="http://purl.obolibrary.org/obo/GAZ_00080541">
        <obo:RO_0001025 rdf:resource="http://purl.obolibrary.org/obo/GAZ_00400056"/>
        <obo:IAO_0000115>A Tehsil in Mianwali District, Punjab.</obo:IAO_0000115>
        <oboInOwl:hasOBONamespace>GAZ</oboInOwl:hasOBONamespace>
        <oboInOwl:id>GAZ:00080541</oboInOwl:id>
        <rdfs:label>Mianwali Teshil</rdfs:label>
    </owl:NamedIndividual>
    


    <!-- http://purl.obolibrary.org/obo/GAZ_00080542 -->

    <owl:NamedIndividual rdf:about="http://purl.obolibrary.org/obo/GAZ_00080542">
        <obo:RO_0001025 rdf:resource="http://purl.obolibrary.org/obo/GAZ_00400053"/>
        <obo:IAO_0000115>A Tehsil in Multan District, Punjab.</obo:IAO_0000115>
        <oboInOwl:hasOBONamespace>GAZ</oboInOwl:hasOBONamespace>
        <oboInOwl:id>GAZ:00080542</oboInOwl:id>
        <rdfs:label>Multan City</rdfs:label>
    </owl:NamedIndividual>
    


    <!-- http://purl.obolibrary.org/obo/GAZ_00080543 -->

    <owl:NamedIndividual rdf:about="http://purl.obolibrary.org/obo/GAZ_00080543">
        <obo:RO_0001025 rdf:resource="http://purl.obolibrary.org/obo/GAZ_00400053"/>
        <obo:IAO_0000115>A Tehsil in Multan District, Punjab.</obo:IAO_0000115>
        <oboInOwl:hasOBONamespace>GAZ</oboInOwl:hasOBONamespace>
        <oboInOwl:id>GAZ:00080543</oboInOwl:id>
        <rdfs:label>Multan Saddar Tehsil</rdfs:label>
    </owl:NamedIndividual>
    


    <!-- http://purl.obolibrary.org/obo/GAZ_00080544 -->

    <owl:NamedIndividual rdf:about="http://purl.obolibrary.org/obo/GAZ_00080544">
        <obo:RO_0001025 rdf:resource="http://purl.obolibrary.org/obo/GAZ_00400053"/>
        <obo:IAO_0000115>A Tehsil in Multan District, Punjab.</obo:IAO_0000115>
        <oboInOwl:hasOBONamespace>GAZ</oboInOwl:hasOBONamespace>
        <oboInOwl:id>GAZ:00080544</oboInOwl:id>
        <rdfs:label>Shujabad Tehsil</rdfs:label>
    </owl:NamedIndividual>
    


    <!-- http://purl.obolibrary.org/obo/GAZ_00080545 -->

    <owl:NamedIndividual rdf:about="http://purl.obolibrary.org/obo/GAZ_00080545">
        <obo:RO_0001025 rdf:resource="http://purl.obolibrary.org/obo/GAZ_00400053"/>
        <obo:IAO_0000115>A Tehsil in Multan District, Punjab.</obo:IAO_0000115>
        <oboInOwl:hasOBONamespace>GAZ</oboInOwl:hasOBONamespace>
        <oboInOwl:id>GAZ:00080545</oboInOwl:id>
        <rdfs:label>Jalalpur Pirwala Tehsil</rdfs:label>
    </owl:NamedIndividual>
    


    <!-- http://purl.obolibrary.org/obo/GAZ_00080546 -->

    <owl:NamedIndividual rdf:about="http://purl.obolibrary.org/obo/GAZ_00080546">
        <obo:RO_0001025 rdf:resource="http://purl.obolibrary.org/obo/GAZ_00400058"/>
        <obo:IAO_0000115>A Tehsil of Muzaffargarh District in the Punjab province of Pakistan.</obo:IAO_0000115>
        <oboInOwl:hasOBONamespace>GAZ</oboInOwl:hasOBONamespace>
        <oboInOwl:id>GAZ:00080546</oboInOwl:id>
        <rdfs:label>Kot Addu Tehsil</rdfs:label>
    </owl:NamedIndividual>
    


    <!-- http://purl.obolibrary.org/obo/GAZ_00080547 -->

    <owl:NamedIndividual rdf:about="http://purl.obolibrary.org/obo/GAZ_00080547">
        <obo:RO_0001025 rdf:resource="http://purl.obolibrary.org/obo/GAZ_00400058"/>
        <obo:IAO_0000115>A Tehsil of Muzaffargarh District in the Punjab province of Pakistan.</obo:IAO_0000115>
        <oboInOwl:hasOBONamespace>GAZ</oboInOwl:hasOBONamespace>
        <oboInOwl:id>GAZ:00080547</oboInOwl:id>
        <rdfs:label>Jatoi Tehsil</rdfs:label>
    </owl:NamedIndividual>
    


    <!-- http://purl.obolibrary.org/obo/GAZ_00080548 -->

    <owl:NamedIndividual rdf:about="http://purl.obolibrary.org/obo/GAZ_00080548">
        <obo:RO_0001025 rdf:resource="http://purl.obolibrary.org/obo/GAZ_00400058"/>
        <obo:IAO_0000115>A Tehsil of Muzaffargarh District in the Punjab province of Pakistan.</obo:IAO_0000115>
        <oboInOwl:hasOBONamespace>GAZ</oboInOwl:hasOBONamespace>
        <oboInOwl:id>GAZ:00080548</oboInOwl:id>
        <rdfs:label>Alipur Tehsil</rdfs:label>
    </owl:NamedIndividual>
    


    <!-- http://purl.obolibrary.org/obo/GAZ_00080549 -->

    <owl:NamedIndividual rdf:about="http://purl.obolibrary.org/obo/GAZ_00080549">
        <obo:RO_0001025 rdf:resource="http://purl.obolibrary.org/obo/GAZ_00400058"/>
        <obo:IAO_0000115>A Tehsil of Muzaffargarh District in the Punjab province of Pakistan.</obo:IAO_0000115>
        <oboInOwl:hasOBONamespace>GAZ</oboInOwl:hasOBONamespace>
        <oboInOwl:id>GAZ:00080549</oboInOwl:id>
        <rdfs:label>Muzaffargarh Tehsil</rdfs:label>
    </owl:NamedIndividual>
    


    <!-- http://purl.obolibrary.org/obo/GAZ_00080550 -->

    <owl:NamedIndividual rdf:about="http://purl.obolibrary.org/obo/GAZ_00080550">
        <obo:RO_0001025 rdf:resource="http://purl.obolibrary.org/obo/GAZ_00400051"/>
        <obo:IAO_0000115>A Tehsil of Narowal District in the Punjab province of Pakistan.</obo:IAO_0000115>
        <oboInOwl:hasOBONamespace>GAZ</oboInOwl:hasOBONamespace>
        <oboInOwl:id>GAZ:00080550</oboInOwl:id>
        <rdfs:label>Narowal Tehsil</rdfs:label>
    </owl:NamedIndividual>
    


    <!-- http://purl.obolibrary.org/obo/GAZ_00080551 -->

    <owl:NamedIndividual rdf:about="http://purl.obolibrary.org/obo/GAZ_00080551">
        <obo:RO_0001025 rdf:resource="http://purl.obolibrary.org/obo/GAZ_00400051"/>
        <obo:IAO_0000115>A Tehsil of Narowal District in the Punjab province of Pakistan.</obo:IAO_0000115>
        <oboInOwl:hasOBONamespace>GAZ</oboInOwl:hasOBONamespace>
        <oboInOwl:id>GAZ:00080551</oboInOwl:id>
        <rdfs:label>Shakargarh Tehsil</rdfs:label>
    </owl:NamedIndividual>
    


    <!-- http://purl.obolibrary.org/obo/GAZ_00080552 -->

    <owl:NamedIndividual rdf:about="http://purl.obolibrary.org/obo/GAZ_00080552">
        <obo:RO_0001025 rdf:resource="http://purl.obolibrary.org/obo/GAZ_00400054"/>
        <obo:IAO_0000115>A Tehsil of Nankana Sahib District, Punjab.</obo:IAO_0000115>
        <oboInOwl:hasOBONamespace>GAZ</oboInOwl:hasOBONamespace>
        <oboInOwl:id>GAZ:00080552</oboInOwl:id>
        <rdfs:label>Sangla Hill Tehsil</rdfs:label>
    </owl:NamedIndividual>
    


    <!-- http://purl.obolibrary.org/obo/GAZ_00080553 -->

    <owl:NamedIndividual rdf:about="http://purl.obolibrary.org/obo/GAZ_00080553">
        <obo:RO_0001025 rdf:resource="http://purl.obolibrary.org/obo/GAZ_00400054"/>
        <obo:IAO_0000115>A Tehsil of Nankana Sahib District, Punjab.</obo:IAO_0000115>
        <oboInOwl:hasOBONamespace>GAZ</oboInOwl:hasOBONamespace>
        <oboInOwl:id>GAZ:00080553</oboInOwl:id>
        <rdfs:label>Safdarabad Tehsil</rdfs:label>
    </owl:NamedIndividual>
    


    <!-- http://purl.obolibrary.org/obo/GAZ_00080554 -->

    <owl:NamedIndividual rdf:about="http://purl.obolibrary.org/obo/GAZ_00080554">
        <obo:RO_0001025 rdf:resource="http://purl.obolibrary.org/obo/GAZ_00400054"/>
        <obo:IAO_0000115>A Tehsil of Nankana Sahib District, Punjab.</obo:IAO_0000115>
        <oboInOwl:hasOBONamespace>GAZ</oboInOwl:hasOBONamespace>
        <oboInOwl:id>GAZ:00080554</oboInOwl:id>
        <rdfs:label>Shahkot Tehsil</rdfs:label>
    </owl:NamedIndividual>
    


    <!-- http://purl.obolibrary.org/obo/GAZ_00080555 -->

    <owl:NamedIndividual rdf:about="http://purl.obolibrary.org/obo/GAZ_00080555">
        <obo:RO_0001025 rdf:resource="http://purl.obolibrary.org/obo/GAZ_00400054"/>
        <obo:IAO_0000115>A Tehsil of Nankana Sahib District, Punjab.</obo:IAO_0000115>
        <oboInOwl:hasOBONamespace>GAZ</oboInOwl:hasOBONamespace>
        <oboInOwl:id>GAZ:00080555</oboInOwl:id>
        <rdfs:label>Nankana Sahib Tehsil</rdfs:label>
    </owl:NamedIndividual>
    


    <!-- http://purl.obolibrary.org/obo/GAZ_00080556 -->

    <owl:NamedIndividual rdf:about="http://purl.obolibrary.org/obo/GAZ_00080556">
        <obo:RO_0001025 rdf:resource="http://purl.obolibrary.org/obo/GAZ_00400055"/>
        <obo:IAO_0000115>A Tehsil in Okara District, Punjab.</obo:IAO_0000115>
        <oboInOwl:hasOBONamespace>GAZ</oboInOwl:hasOBONamespace>
        <oboInOwl:id>GAZ:00080556</oboInOwl:id>
        <rdfs:label>Renala Khurd Tehsil</rdfs:label>
    </owl:NamedIndividual>
    


    <!-- http://purl.obolibrary.org/obo/GAZ_00080557 -->

    <owl:NamedIndividual rdf:about="http://purl.obolibrary.org/obo/GAZ_00080557">
        <obo:RO_0001025 rdf:resource="http://purl.obolibrary.org/obo/GAZ_00400055"/>
        <obo:IAO_0000115>A Tehsil in Okara District, Punjab.</obo:IAO_0000115>
        <oboInOwl:hasOBONamespace>GAZ</oboInOwl:hasOBONamespace>
        <oboInOwl:id>GAZ:00080557</oboInOwl:id>
        <rdfs:label>Depalpur Tehsil</rdfs:label>
    </owl:NamedIndividual>
    


    <!-- http://purl.obolibrary.org/obo/GAZ_00080558 -->

    <owl:NamedIndividual rdf:about="http://purl.obolibrary.org/obo/GAZ_00080558">
        <obo:RO_0001025 rdf:resource="http://purl.obolibrary.org/obo/GAZ_00400055"/>
        <obo:IAO_0000115>A Tehsil in Okara District, Punjab.</obo:IAO_0000115>
        <oboInOwl:hasOBONamespace>GAZ</oboInOwl:hasOBONamespace>
        <oboInOwl:id>GAZ:00080558</oboInOwl:id>
        <rdfs:label>Okara Tehsil</rdfs:label>
    </owl:NamedIndividual>
    


    <!-- http://purl.obolibrary.org/obo/GAZ_00080559 -->

    <owl:NamedIndividual rdf:about="http://purl.obolibrary.org/obo/GAZ_00080559">
        <obo:RO_0001025 rdf:resource="http://purl.obolibrary.org/obo/GAZ_00400059"/>
        <obo:IAO_0000115>A Tehsil of Pakpattan District in the Punjab province of Pakistan.</obo:IAO_0000115>
        <oboInOwl:hasOBONamespace>GAZ</oboInOwl:hasOBONamespace>
        <oboInOwl:id>GAZ:00080559</oboInOwl:id>
        <rdfs:label>Arifwala Tehsil</rdfs:label>
    </owl:NamedIndividual>
    


    <!-- http://purl.obolibrary.org/obo/GAZ_00080560 -->

    <owl:NamedIndividual rdf:about="http://purl.obolibrary.org/obo/GAZ_00080560">
        <obo:RO_0001025 rdf:resource="http://purl.obolibrary.org/obo/GAZ_00400059"/>
        <obo:IAO_0000115>A Tehsil of Pakpattan District in the Punjab province of Pakistan.</obo:IAO_0000115>
        <oboInOwl:hasOBONamespace>GAZ</oboInOwl:hasOBONamespace>
        <oboInOwl:id>GAZ:00080560</oboInOwl:id>
        <rdfs:label>Pakpattan Tehsil</rdfs:label>
    </owl:NamedIndividual>
    


    <!-- http://purl.obolibrary.org/obo/GAZ_00080561 -->

    <owl:NamedIndividual rdf:about="http://purl.obolibrary.org/obo/GAZ_00080561">
        <obo:RO_0001025 rdf:resource="http://purl.obolibrary.org/obo/GAZ_00400057"/>
        <obo:IAO_0000115>A Tehsil of Rahimyar Khan District in the Punjab province of Pakistan.</obo:IAO_0000115>
        <oboInOwl:hasOBONamespace>GAZ</oboInOwl:hasOBONamespace>
        <oboInOwl:id>GAZ:00080561</oboInOwl:id>
        <rdfs:label>Sadiqabad Tehsil</rdfs:label>
    </owl:NamedIndividual>
    


    <!-- http://purl.obolibrary.org/obo/GAZ_00080562 -->

    <owl:NamedIndividual rdf:about="http://purl.obolibrary.org/obo/GAZ_00080562">
        <obo:RO_0001025 rdf:resource="http://purl.obolibrary.org/obo/GAZ_00400057"/>
        <obo:IAO_0000115>A Tehsil of Rahimyar Khan District in the Punjab province of Pakistan.</obo:IAO_0000115>
        <oboInOwl:hasOBONamespace>GAZ</oboInOwl:hasOBONamespace>
        <oboInOwl:id>GAZ:00080562</oboInOwl:id>
        <rdfs:label>Rahim Yar Khan Teshil</rdfs:label>
    </owl:NamedIndividual>
    


    <!-- http://purl.obolibrary.org/obo/GAZ_00080563 -->

    <owl:NamedIndividual rdf:about="http://purl.obolibrary.org/obo/GAZ_00080563">
        <obo:RO_0001025 rdf:resource="http://purl.obolibrary.org/obo/GAZ_00400057"/>
        <obo:IAO_0000115>A Tehsil of Rahimyar Khan District in the Punjab province of Pakistan.</obo:IAO_0000115>
        <oboInOwl:hasOBONamespace>GAZ</oboInOwl:hasOBONamespace>
        <oboInOwl:id>GAZ:00080563</oboInOwl:id>
        <rdfs:label>Liaquatpur Tehsil</rdfs:label>
    </owl:NamedIndividual>
    


    <!-- http://purl.obolibrary.org/obo/GAZ_00080564 -->

    <owl:NamedIndividual rdf:about="http://purl.obolibrary.org/obo/GAZ_00080564">
        <obo:RO_0001025 rdf:resource="http://purl.obolibrary.org/obo/GAZ_00400057"/>
        <obo:IAO_0000115>A Tehsil of Rahimyar Khan District in the Punjab province of Pakistan.</obo:IAO_0000115>
        <oboInOwl:hasOBONamespace>GAZ</oboInOwl:hasOBONamespace>
        <oboInOwl:id>GAZ:00080564</oboInOwl:id>
        <rdfs:label>Khanpur Tehsil</rdfs:label>
    </owl:NamedIndividual>
    


    <!-- http://purl.obolibrary.org/obo/GAZ_00080565 -->

    <owl:NamedIndividual rdf:about="http://purl.obolibrary.org/obo/GAZ_00080565">
        <obo:RO_0001025 rdf:resource="http://purl.obolibrary.org/obo/GAZ_00400050"/>
        <obo:IAO_0000115>A Tehsil in Rajanpur District, Punjab.</obo:IAO_0000115>
        <oboInOwl:hasOBONamespace>GAZ</oboInOwl:hasOBONamespace>
        <oboInOwl:id>GAZ:00080565</oboInOwl:id>
        <rdfs:label>Rojhan Tehsil</rdfs:label>
    </owl:NamedIndividual>
    


    <!-- http://purl.obolibrary.org/obo/GAZ_00080566 -->

    <owl:NamedIndividual rdf:about="http://purl.obolibrary.org/obo/GAZ_00080566">
        <obo:RO_0001025 rdf:resource="http://purl.obolibrary.org/obo/GAZ_00400050"/>
        <obo:IAO_0000115>A Tehsil in Rajanpur District, Punjab.</obo:IAO_0000115>
        <oboInOwl:hasOBONamespace>GAZ</oboInOwl:hasOBONamespace>
        <oboInOwl:id>GAZ:00080566</oboInOwl:id>
        <rdfs:label>Rajanpur Tehsil</rdfs:label>
    </owl:NamedIndividual>
    


    <!-- http://purl.obolibrary.org/obo/GAZ_00080567 -->

    <owl:NamedIndividual rdf:about="http://purl.obolibrary.org/obo/GAZ_00080567">
        <obo:RO_0001025 rdf:resource="http://purl.obolibrary.org/obo/GAZ_00400050"/>
        <obo:IAO_0000115>A Tehsil in Rajanpur District, Punjab.</obo:IAO_0000115>
        <oboInOwl:hasOBONamespace>GAZ</oboInOwl:hasOBONamespace>
        <oboInOwl:id>GAZ:00080567</oboInOwl:id>
        <rdfs:label>Jampur Tehsil</rdfs:label>
    </owl:NamedIndividual>
    


    <!-- http://purl.obolibrary.org/obo/GAZ_00080568 -->

    <owl:NamedIndividual rdf:about="http://purl.obolibrary.org/obo/GAZ_00080568">
        <obo:RO_0001025 rdf:resource="http://purl.obolibrary.org/obo/GAZ_00400062"/>
        <obo:IAO_0000115>A Tehsil in Sahiwal District, Punjab.</obo:IAO_0000115>
        <oboInOwl:hasOBONamespace>GAZ</oboInOwl:hasOBONamespace>
        <oboInOwl:id>GAZ:00080568</oboInOwl:id>
        <rdfs:label>Sahiwal Tehsil</rdfs:label>
    </owl:NamedIndividual>
    


    <!-- http://purl.obolibrary.org/obo/GAZ_00080569 -->

    <owl:NamedIndividual rdf:about="http://purl.obolibrary.org/obo/GAZ_00080569">
        <obo:RO_0001025 rdf:resource="http://purl.obolibrary.org/obo/GAZ_00400062"/>
        <obo:IAO_0000115>A Tehsil in Sahiwal District, Punjab.</obo:IAO_0000115>
        <oboInOwl:hasOBONamespace>GAZ</oboInOwl:hasOBONamespace>
        <oboInOwl:id>GAZ:00080569</oboInOwl:id>
        <rdfs:label>Chichawatni Tehsil</rdfs:label>
    </owl:NamedIndividual>
    


    <!-- http://purl.obolibrary.org/obo/GAZ_00080570 -->

    <owl:NamedIndividual rdf:about="http://purl.obolibrary.org/obo/GAZ_00080570">
        <obo:RO_0001025 rdf:resource="http://purl.obolibrary.org/obo/GAZ_00400052"/>
        <obo:IAO_0000115>A Tehsil of Vehari District, Punjab.</obo:IAO_0000115>
        <oboInOwl:hasOBONamespace>GAZ</oboInOwl:hasOBONamespace>
        <oboInOwl:id>GAZ:00080570</oboInOwl:id>
        <rdfs:label>Vehari Tehsil</rdfs:label>
    </owl:NamedIndividual>
    


    <!-- http://purl.obolibrary.org/obo/GAZ_00080571 -->

    <owl:NamedIndividual rdf:about="http://purl.obolibrary.org/obo/GAZ_00080571">
        <obo:RO_0001025 rdf:resource="http://purl.obolibrary.org/obo/GAZ_00400052"/>
        <obo:IAO_0000115>A Tehsil of Vehari District, Punjab.</obo:IAO_0000115>
        <oboInOwl:hasOBONamespace>GAZ</oboInOwl:hasOBONamespace>
        <oboInOwl:id>GAZ:00080571</oboInOwl:id>
        <rdfs:label>Burewala Tehsil</rdfs:label>
    </owl:NamedIndividual>
    


    <!-- http://purl.obolibrary.org/obo/GAZ_00080572 -->

    <owl:NamedIndividual rdf:about="http://purl.obolibrary.org/obo/GAZ_00080572">
        <obo:RO_0001025 rdf:resource="http://purl.obolibrary.org/obo/GAZ_00400052"/>
        <obo:IAO_0000115>A Tehsil of Vehari District, Punjab.</obo:IAO_0000115>
        <oboInOwl:hasOBONamespace>GAZ</oboInOwl:hasOBONamespace>
        <oboInOwl:id>GAZ:00080572</oboInOwl:id>
        <rdfs:label>Mailsi Tehsil</rdfs:label>
    </owl:NamedIndividual>
    


    <!-- http://purl.obolibrary.org/obo/GAZ_00080573 -->

    <owl:NamedIndividual rdf:about="http://purl.obolibrary.org/obo/GAZ_00080573">
        <obo:RO_0001025 rdf:resource="http://purl.obolibrary.org/obo/GAZ_00400064"/>
        <obo:IAO_0000115>A Tehsil of Toba Tek Singh District in the Punjab province of Pakistan.</obo:IAO_0000115>
        <oboInOwl:hasOBONamespace>GAZ</oboInOwl:hasOBONamespace>
        <oboInOwl:id>GAZ:00080573</oboInOwl:id>
        <rdfs:label>Toba Tek Singh Tehsil</rdfs:label>
    </owl:NamedIndividual>
    


    <!-- http://purl.obolibrary.org/obo/GAZ_00080574 -->

    <owl:NamedIndividual rdf:about="http://purl.obolibrary.org/obo/GAZ_00080574">
        <obo:RO_0001025 rdf:resource="http://purl.obolibrary.org/obo/GAZ_00400064"/>
        <obo:IAO_0000115>A Tehsil of Toba Tek Singh District in the Punjab province of Pakistan.</obo:IAO_0000115>
        <oboInOwl:hasOBONamespace>GAZ</oboInOwl:hasOBONamespace>
        <oboInOwl:id>GAZ:00080574</oboInOwl:id>
        <rdfs:label>Kamalia Tehsil</rdfs:label>
    </owl:NamedIndividual>
    


    <!-- http://purl.obolibrary.org/obo/GAZ_00080575 -->

    <owl:NamedIndividual rdf:about="http://purl.obolibrary.org/obo/GAZ_00080575">
        <obo:RO_0001025 rdf:resource="http://purl.obolibrary.org/obo/GAZ_00400064"/>
        <obo:IAO_0000115>A Tehsil of Toba Tek Singh District in the Punjab province of Pakistan.</obo:IAO_0000115>
        <oboInOwl:hasOBONamespace>GAZ</oboInOwl:hasOBONamespace>
        <oboInOwl:id>GAZ:00080575</oboInOwl:id>
        <rdfs:label>Gojra Tehsil</rdfs:label>
    </owl:NamedIndividual>
    


    <!-- http://purl.obolibrary.org/obo/GAZ_00080576 -->

    <owl:NamedIndividual rdf:about="http://purl.obolibrary.org/obo/GAZ_00080576">
        <obo:RO_0001025 rdf:resource="http://purl.obolibrary.org/obo/GAZ_00400063"/>
        <obo:IAO_0000115>A small industrial city in the Punjab province of Pakistan. The town has the status of Tehsil (Sub District) and is one of four Tehsils of district Sialkot.</obo:IAO_0000115>
        <oboInOwl:hasOBONamespace>GAZ</oboInOwl:hasOBONamespace>
        <oboInOwl:id>GAZ:00080576</oboInOwl:id>
        <rdfs:label>Daska Teshil</rdfs:label>
    </owl:NamedIndividual>
    


    <!-- http://purl.obolibrary.org/obo/GAZ_00080577 -->

    <owl:NamedIndividual rdf:about="http://purl.obolibrary.org/obo/GAZ_00080577">
        <obo:RO_0001025 rdf:resource="http://purl.obolibrary.org/obo/GAZ_00400063"/>
        <obo:IAO_0000115>A Tehsil of Sialkot District in the Punjab province of Pakistan.</obo:IAO_0000115>
        <oboInOwl:hasOBONamespace>GAZ</oboInOwl:hasOBONamespace>
        <oboInOwl:id>GAZ:00080577</oboInOwl:id>
        <rdfs:label>Pasrur Tehsil</rdfs:label>
    </owl:NamedIndividual>
    


    <!-- http://purl.obolibrary.org/obo/GAZ_00080578 -->

    <owl:NamedIndividual rdf:about="http://purl.obolibrary.org/obo/GAZ_00080578">
        <obo:RO_0001025 rdf:resource="http://purl.obolibrary.org/obo/GAZ_00400063"/>
        <obo:IAO_0000115>A Tehsil of Sialkot District in the Punjab province of Pakistan.</obo:IAO_0000115>
        <oboInOwl:hasOBONamespace>GAZ</oboInOwl:hasOBONamespace>
        <oboInOwl:id>GAZ:00080578</oboInOwl:id>
        <rdfs:label>Sialkot Tehsil</rdfs:label>
    </owl:NamedIndividual>
    


    <!-- http://purl.obolibrary.org/obo/GAZ_00080579 -->

    <owl:NamedIndividual rdf:about="http://purl.obolibrary.org/obo/GAZ_00080579">
        <obo:RO_0001025 rdf:resource="http://purl.obolibrary.org/obo/GAZ_00400063"/>
        <obo:IAO_0000115>A Tehsil of Sialkot District in the Punjab province of Pakistan.</obo:IAO_0000115>
        <oboInOwl:hasOBONamespace>GAZ</oboInOwl:hasOBONamespace>
        <oboInOwl:id>GAZ:00080579</oboInOwl:id>
        <rdfs:label>Sambrial Tehsil</rdfs:label>
    </owl:NamedIndividual>
    


    <!-- http://purl.obolibrary.org/obo/GAZ_00080580 -->

    <owl:NamedIndividual rdf:about="http://purl.obolibrary.org/obo/GAZ_00080580">
        <obo:RO_0001025 rdf:resource="http://purl.obolibrary.org/obo/GAZ_00400061"/>
        <obo:IAO_0000115>A Tehsil in Sheikhupura District, Punjab.</obo:IAO_0000115>
        <oboInOwl:hasOBONamespace>GAZ</oboInOwl:hasOBONamespace>
        <oboInOwl:id>GAZ:00080580</oboInOwl:id>
        <rdfs:label>Ferozewala Tehsil</rdfs:label>
    </owl:NamedIndividual>
    


    <!-- http://purl.obolibrary.org/obo/GAZ_00080581 -->

    <owl:NamedIndividual rdf:about="http://purl.obolibrary.org/obo/GAZ_00080581">
        <obo:RO_0001025 rdf:resource="http://purl.obolibrary.org/obo/GAZ_00400061"/>
        <obo:IAO_0000115>A Tehsil in Sheikhupura District, Punjab.</obo:IAO_0000115>
        <oboInOwl:hasOBONamespace>GAZ</oboInOwl:hasOBONamespace>
        <oboInOwl:id>GAZ:00080581</oboInOwl:id>
        <rdfs:label>Sheikhupura Tehsil</rdfs:label>
    </owl:NamedIndividual>
    


    <!-- http://purl.obolibrary.org/obo/GAZ_00080582 -->

    <owl:NamedIndividual rdf:about="http://purl.obolibrary.org/obo/GAZ_00080582">
        <obo:RO_0001025 rdf:resource="http://purl.obolibrary.org/obo/GAZ_00400061"/>
        <obo:IAO_0000115>A Tehsil in Sheikhupura District, Punjab.</obo:IAO_0000115>
        <oboInOwl:hasOBONamespace>GAZ</oboInOwl:hasOBONamespace>
        <oboInOwl:id>GAZ:00080582</oboInOwl:id>
        <rdfs:label>Sharaqpur Tehsil</rdfs:label>
    </owl:NamedIndividual>
    


    <!-- http://purl.obolibrary.org/obo/GAZ_00080583 -->

    <owl:NamedIndividual rdf:about="http://purl.obolibrary.org/obo/GAZ_00080583">
        <obo:RO_0001025 rdf:resource="http://purl.obolibrary.org/obo/GAZ_00400061"/>
        <obo:IAO_0000115>A Tehsil in Sheikhupura District, Punjab.</obo:IAO_0000115>
        <oboInOwl:hasOBONamespace>GAZ</oboInOwl:hasOBONamespace>
        <oboInOwl:id>GAZ:00080583</oboInOwl:id>
        <rdfs:label>Muridke Tehsil</rdfs:label>
    </owl:NamedIndividual>
    


    <!-- http://purl.obolibrary.org/obo/GAZ_00080584 -->

    <owl:NamedIndividual rdf:about="http://purl.obolibrary.org/obo/GAZ_00080584">
        <obo:RO_0001025 rdf:resource="http://purl.obolibrary.org/obo/GAZ_00400060"/>
        <obo:IAO_0000115>A Tehsil of Sargodha District in the Punjab province of Pakistan.</obo:IAO_0000115>
        <oboInOwl:hasOBONamespace>GAZ</oboInOwl:hasOBONamespace>
        <oboInOwl:id>GAZ:00080584</oboInOwl:id>
        <rdfs:label>Sillanwali Tehsil</rdfs:label>
    </owl:NamedIndividual>
    


    <!-- http://purl.obolibrary.org/obo/GAZ_00080585 -->

    <owl:NamedIndividual rdf:about="http://purl.obolibrary.org/obo/GAZ_00080585">
        <obo:RO_0001025 rdf:resource="http://purl.obolibrary.org/obo/GAZ_00400060"/>
        <obo:IAO_0000115>A Tehsil of Sargodha District in the Punjab province of Pakistan.</obo:IAO_0000115>
        <oboInOwl:hasOBONamespace>GAZ</oboInOwl:hasOBONamespace>
        <oboInOwl:id>GAZ:00080585</oboInOwl:id>
        <rdfs:label>Shahpur Tehsil</rdfs:label>
    </owl:NamedIndividual>
    


    <!-- http://purl.obolibrary.org/obo/GAZ_00080586 -->

    <owl:NamedIndividual rdf:about="http://purl.obolibrary.org/obo/GAZ_00080586">
        <obo:RO_0001025 rdf:resource="http://purl.obolibrary.org/obo/GAZ_00400060"/>
        <obo:IAO_0000115>A Tehsil of Sargodha District in the Punjab province of Pakistan.</obo:IAO_0000115>
        <oboInOwl:hasOBONamespace>GAZ</oboInOwl:hasOBONamespace>
        <oboInOwl:id>GAZ:00080586</oboInOwl:id>
        <rdfs:label>Bhalwal Tehsil</rdfs:label>
    </owl:NamedIndividual>
    


    <!-- http://purl.obolibrary.org/obo/GAZ_00080587 -->

    <owl:NamedIndividual rdf:about="http://purl.obolibrary.org/obo/GAZ_00080587">
        <obo:RO_0001025 rdf:resource="http://purl.obolibrary.org/obo/GAZ_00400060"/>
        <obo:IAO_0000115>A Tehsil of Sargodha District in the Punjab province of Pakistan.</obo:IAO_0000115>
        <oboInOwl:hasOBONamespace>GAZ</oboInOwl:hasOBONamespace>
        <oboInOwl:id>GAZ:00080587</oboInOwl:id>
        <rdfs:label>Sahiwal Tehsil</rdfs:label>
    </owl:NamedIndividual>
    


    <!-- http://purl.obolibrary.org/obo/GAZ_00080588 -->

    <owl:NamedIndividual rdf:about="http://purl.obolibrary.org/obo/GAZ_00080588">
        <obo:RO_0001025 rdf:resource="http://purl.obolibrary.org/obo/GAZ_00400060"/>
        <obo:IAO_0000115>A Tehsil of Sargodha District in the Punjab province of Pakistan.</obo:IAO_0000115>
        <oboInOwl:hasOBONamespace>GAZ</oboInOwl:hasOBONamespace>
        <oboInOwl:id>GAZ:00080588</oboInOwl:id>
        <rdfs:label>Sargodha Tehsil</rdfs:label>
    </owl:NamedIndividual>
    


    <!-- http://purl.obolibrary.org/obo/GAZ_00080589 -->

    <owl:NamedIndividual rdf:about="http://purl.obolibrary.org/obo/GAZ_00080589">
        <obo:RO_0001025 rdf:resource="http://purl.obolibrary.org/obo/GAZ_00018569"/>
        <obo:IAO_0000115>A Tehsil of Bhimber District, Azad Kashmir.</obo:IAO_0000115>
        <oboInOwl:hasOBONamespace>GAZ</oboInOwl:hasOBONamespace>
        <oboInOwl:id>GAZ:00080589</oboInOwl:id>
        <rdfs:label>Bhimber Tehsil</rdfs:label>
    </owl:NamedIndividual>
    


    <!-- http://purl.obolibrary.org/obo/GAZ_00080590 -->

    <owl:NamedIndividual rdf:about="http://purl.obolibrary.org/obo/GAZ_00080590">
        <obo:RO_0001025 rdf:resource="http://purl.obolibrary.org/obo/GAZ_00018569"/>
        <obo:IAO_0000115>A Tehsil of Bhimber District, Azad Kashmir.</obo:IAO_0000115>
        <oboInOwl:hasOBONamespace>GAZ</oboInOwl:hasOBONamespace>
        <oboInOwl:id>GAZ:00080590</oboInOwl:id>
        <rdfs:label>Barnala Tehsil</rdfs:label>
    </owl:NamedIndividual>
    


    <!-- http://purl.obolibrary.org/obo/GAZ_00080591 -->

    <owl:NamedIndividual rdf:about="http://purl.obolibrary.org/obo/GAZ_00080591">
        <obo:RO_0001025 rdf:resource="http://purl.obolibrary.org/obo/GAZ_00018569"/>
        <obo:IAO_0000115>A Tehsil of Bhimber District, Azad Kashmir.</obo:IAO_0000115>
        <oboInOwl:hasOBONamespace>GAZ</oboInOwl:hasOBONamespace>
        <oboInOwl:id>GAZ:00080591</oboInOwl:id>
        <rdfs:label>Samahni Tehsil</rdfs:label>
    </owl:NamedIndividual>
    


    <!-- http://purl.obolibrary.org/obo/GAZ_00080592 -->

    <owl:NamedIndividual rdf:about="http://purl.obolibrary.org/obo/GAZ_00080592">
        <obo:RO_0001025 rdf:resource="http://purl.obolibrary.org/obo/GAZ_00018567"/>
        <obo:IAO_0000115>A Tehsil of Kotli District, Azad Kashmir, Pakistan.</obo:IAO_0000115>
        <oboInOwl:hasOBONamespace>GAZ</oboInOwl:hasOBONamespace>
        <oboInOwl:id>GAZ:00080592</oboInOwl:id>
        <rdfs:label>Kotli Tehsil</rdfs:label>
    </owl:NamedIndividual>
    


    <!-- http://purl.obolibrary.org/obo/GAZ_00080593 -->

    <owl:NamedIndividual rdf:about="http://purl.obolibrary.org/obo/GAZ_00080593">
        <obo:RO_0001025 rdf:resource="http://purl.obolibrary.org/obo/GAZ_00018567"/>
        <obo:IAO_0000115>A Tehsil of Kotli District, Azad Kashmir, Pakistan. Nakyal was part of Mehndar sub-division of Poonch before the division of Kashmir in 1947. After the separation from Mehndar it became a tehsil of Kotli District.</obo:IAO_0000115>
        <oboInOwl:hasOBONamespace>GAZ</oboInOwl:hasOBONamespace>
        <oboInOwl:id>GAZ:00080593</oboInOwl:id>
        <rdfs:label>Nakyal Tehsil</rdfs:label>
    </owl:NamedIndividual>
    


    <!-- http://purl.obolibrary.org/obo/GAZ_00080594 -->

    <owl:NamedIndividual rdf:about="http://purl.obolibrary.org/obo/GAZ_00080594">
        <obo:RO_0001025 rdf:resource="http://purl.obolibrary.org/obo/GAZ_00018567"/>
        <obo:IAO_0000115>A Tehsil of Kotli District, Azad Kashmir, Pakistan.</obo:IAO_0000115>
        <oboInOwl:hasOBONamespace>GAZ</oboInOwl:hasOBONamespace>
        <oboInOwl:id>GAZ:00080594</oboInOwl:id>
        <rdfs:label>Sehnsa Tehsil</rdfs:label>
    </owl:NamedIndividual>
    


    <!-- http://purl.obolibrary.org/obo/GAZ_00080595 -->

    <owl:NamedIndividual rdf:about="http://purl.obolibrary.org/obo/GAZ_00080595">
        <obo:RO_0001025 rdf:resource="http://purl.obolibrary.org/obo/GAZ_00018568"/>
        <obo:IAO_0000115>A Tehsil in Mirpur District, Azad Kashmir.</obo:IAO_0000115>
        <oboInOwl:hasOBONamespace>GAZ</oboInOwl:hasOBONamespace>
        <oboInOwl:id>GAZ:00080595</oboInOwl:id>
        <rdfs:label>Chakswari Tehsil</rdfs:label>
    </owl:NamedIndividual>
    


    <!-- http://purl.obolibrary.org/obo/GAZ_00080596 -->

    <owl:NamedIndividual rdf:about="http://purl.obolibrary.org/obo/GAZ_00080596">
        <obo:RO_0001025 rdf:resource="http://purl.obolibrary.org/obo/GAZ_00018568"/>
        <obo:IAO_0000115>A Tehsil in Mirpur District, Azad Kashmir.</obo:IAO_0000115>
        <oboInOwl:hasOBONamespace>GAZ</oboInOwl:hasOBONamespace>
        <oboInOwl:id>GAZ:00080596</oboInOwl:id>
        <rdfs:label>Mirpur City</rdfs:label>
    </owl:NamedIndividual>
    


    <!-- http://purl.obolibrary.org/obo/GAZ_00080597 -->

    <owl:NamedIndividual rdf:about="http://purl.obolibrary.org/obo/GAZ_00080597">
        <obo:RO_0001025 rdf:resource="http://purl.obolibrary.org/obo/GAZ_00018568"/>
        <obo:IAO_0000115>A Tehsil in Mirpur District, Azad Kashmir.</obo:IAO_0000115>
        <oboInOwl:hasOBONamespace>GAZ</oboInOwl:hasOBONamespace>
        <oboInOwl:id>GAZ:00080597</oboInOwl:id>
        <rdfs:label>Dudial Tehsil</rdfs:label>
    </owl:NamedIndividual>
    


    <!-- http://purl.obolibrary.org/obo/GAZ_00080598 -->

    <owl:NamedIndividual rdf:about="http://purl.obolibrary.org/obo/GAZ_00080598">
        <obo:RO_0001025 rdf:resource="http://purl.obolibrary.org/obo/GAZ_00018571"/>
        <obo:IAO_0000115>A Tehsil of Sudhnati District, Azad Kashmir.</obo:IAO_0000115>
        <oboInOwl:hasOBONamespace>GAZ</oboInOwl:hasOBONamespace>
        <oboInOwl:id>GAZ:00080598</oboInOwl:id>
        <rdfs:label>Balouch Tehsil</rdfs:label>
    </owl:NamedIndividual>
    


    <!-- http://purl.obolibrary.org/obo/GAZ_00080599 -->

    <owl:NamedIndividual rdf:about="http://purl.obolibrary.org/obo/GAZ_00080599">
        <obo:RO_0001025 rdf:resource="http://purl.obolibrary.org/obo/GAZ_00018571"/>
        <obo:IAO_0000115>A Tehsil of Sudhnati District, Azad Kashmir.</obo:IAO_0000115>
        <oboInOwl:hasOBONamespace>GAZ</oboInOwl:hasOBONamespace>
        <oboInOwl:id>GAZ:00080599</oboInOwl:id>
        <rdfs:label>Trarkhal Tehsil</rdfs:label>
    </owl:NamedIndividual>
    


    <!-- http://purl.obolibrary.org/obo/GAZ_00080600 -->

    <owl:NamedIndividual rdf:about="http://purl.obolibrary.org/obo/GAZ_00080600">
        <obo:RO_0001025 rdf:resource="http://purl.obolibrary.org/obo/GAZ_00018573"/>
        <obo:IAO_0000115>A Tehsil of Neelum District, Azad Kashmir.</obo:IAO_0000115>
        <oboInOwl:hasOBONamespace>GAZ</oboInOwl:hasOBONamespace>
        <oboInOwl:id>GAZ:00080600</oboInOwl:id>
        <rdfs:label>Athmuuqaam Tehsil</rdfs:label>
    </owl:NamedIndividual>
    


    <!-- http://purl.obolibrary.org/obo/GAZ_00080601 -->

    <owl:NamedIndividual rdf:about="http://purl.obolibrary.org/obo/GAZ_00080601">
        <obo:RO_0001025 rdf:resource="http://purl.obolibrary.org/obo/GAZ_00018573"/>
        <obo:IAO_0000115>A Tehsil of Neelum District, Azad Kashmir.</obo:IAO_0000115>
        <oboInOwl:hasOBONamespace>GAZ</oboInOwl:hasOBONamespace>
        <oboInOwl:id>GAZ:00080601</oboInOwl:id>
        <rdfs:label>Sharda Tehsil</rdfs:label>
    </owl:NamedIndividual>
    


    <!-- http://purl.obolibrary.org/obo/GAZ_00080602 -->

    <owl:NamedIndividual rdf:about="http://purl.obolibrary.org/obo/GAZ_00080602">
        <obo:RO_0001025 rdf:resource="http://purl.obolibrary.org/obo/GAZ_00018572"/>
        <obo:IAO_0000115>A Tehsil of Muzaffarabad District, Azur Kashmir.</obo:IAO_0000115>
        <oboInOwl:hasOBONamespace>GAZ</oboInOwl:hasOBONamespace>
        <oboInOwl:id>GAZ:00080602</oboInOwl:id>
        <rdfs:label>Muzaffarabad Tehsil</rdfs:label>
    </owl:NamedIndividual>
    


    <!-- http://purl.obolibrary.org/obo/GAZ_00080603 -->

    <owl:NamedIndividual rdf:about="http://purl.obolibrary.org/obo/GAZ_00080603">
        <obo:RO_0001025 rdf:resource="http://purl.obolibrary.org/obo/GAZ_00018572"/>
        <obo:IAO_0000115>A Tehsil of Muzaffarabad District, Azur Kashmir.</obo:IAO_0000115>
        <oboInOwl:hasOBONamespace>GAZ</oboInOwl:hasOBONamespace>
        <oboInOwl:id>GAZ:00080603</oboInOwl:id>
        <rdfs:label>Hattian Pattika Tehsil</rdfs:label>
    </owl:NamedIndividual>
    


    <!-- http://purl.obolibrary.org/obo/GAZ_00080604 -->

    <owl:NamedIndividual rdf:about="http://purl.obolibrary.org/obo/GAZ_00080604">
        <obo:RO_0001025 rdf:resource="http://purl.obolibrary.org/obo/GAZ_00018574"/>
        <obo:IAO_0000115>A Tehsil of Bagh District, Azad Kashmir.</obo:IAO_0000115>
        <oboInOwl:hasOBONamespace>GAZ</oboInOwl:hasOBONamespace>
        <oboInOwl:id>GAZ:00080604</oboInOwl:id>
        <rdfs:label>Hawailee Tehsil</rdfs:label>
    </owl:NamedIndividual>
    


    <!-- http://purl.obolibrary.org/obo/GAZ_00080605 -->

    <owl:NamedIndividual rdf:about="http://purl.obolibrary.org/obo/GAZ_00080605">
        <obo:RO_0001025 rdf:resource="http://purl.obolibrary.org/obo/GAZ_00018571"/>
        <obo:IAO_0000115>A Tehsil of Sudhnati District, Azad Kashmir.</obo:IAO_0000115>
        <oboInOwl:hasOBONamespace>GAZ</oboInOwl:hasOBONamespace>
        <oboInOwl:id>GAZ:00080605</oboInOwl:id>
        <rdfs:label>Mong Tehsil</rdfs:label>
    </owl:NamedIndividual>
    


    <!-- http://purl.obolibrary.org/obo/GAZ_00080606 -->

    <owl:NamedIndividual rdf:about="http://purl.obolibrary.org/obo/GAZ_00080606">
        <obo:RO_0001025 rdf:resource="http://purl.obolibrary.org/obo/GAZ_00018574"/>
        <obo:IAO_0000115>A Tehsil of Bagh District, Azad Kashmir.</obo:IAO_0000115>
        <oboInOwl:hasOBONamespace>GAZ</oboInOwl:hasOBONamespace>
        <oboInOwl:id>GAZ:00080606</oboInOwl:id>
        <rdfs:label>Bagh Tehsil</rdfs:label>
    </owl:NamedIndividual>
    


    <!-- http://purl.obolibrary.org/obo/GAZ_00080607 -->

    <owl:NamedIndividual rdf:about="http://purl.obolibrary.org/obo/GAZ_00080607">
        <obo:RO_0001025 rdf:resource="http://purl.obolibrary.org/obo/GAZ_00018574"/>
        <obo:IAO_0000115>A Tehsil of Bagh District, Azad Kashmir.</obo:IAO_0000115>
        <oboInOwl:hasOBONamespace>GAZ</oboInOwl:hasOBONamespace>
        <oboInOwl:id>GAZ:00080607</oboInOwl:id>
        <rdfs:label>Dhirkot Tehsil</rdfs:label>
    </owl:NamedIndividual>
    


    <!-- http://purl.obolibrary.org/obo/GAZ_00080608 -->

    <owl:NamedIndividual rdf:about="http://purl.obolibrary.org/obo/GAZ_00080608">
        <obo:RO_0001025 rdf:resource="http://purl.obolibrary.org/obo/GAZ_00018562"/>
        <obo:IAO_0000115>A subdivision of the Khyber Agency.</obo:IAO_0000115>
        <oboInOwl:hasOBONamespace>GAZ</oboInOwl:hasOBONamespace>
        <oboInOwl:id>GAZ:00080608</oboInOwl:id>
        <rdfs:label>Jamrud Subdivision</rdfs:label>
    </owl:NamedIndividual>
    


    <!-- http://purl.obolibrary.org/obo/GAZ_00080609 -->

    <owl:NamedIndividual rdf:about="http://purl.obolibrary.org/obo/GAZ_00080609">
        <obo:RO_0001025 rdf:resource="http://purl.obolibrary.org/obo/GAZ_00018562"/>
        <obo:IAO_0000115>A subdivision of the Khyber Agency.</obo:IAO_0000115>
        <oboInOwl:hasOBONamespace>GAZ</oboInOwl:hasOBONamespace>
        <oboInOwl:id>GAZ:00080609</oboInOwl:id>
        <rdfs:label>Bara Subdivision</rdfs:label>
    </owl:NamedIndividual>
    


    <!-- http://purl.obolibrary.org/obo/GAZ_00080610 -->

    <owl:NamedIndividual rdf:about="http://purl.obolibrary.org/obo/GAZ_00080610">
        <obo:RO_0001025 rdf:resource="http://purl.obolibrary.org/obo/GAZ_00018562"/>
        <obo:IAO_0000115>A subdivision of the Khyber Agency.</obo:IAO_0000115>
        <oboInOwl:hasOBONamespace>GAZ</oboInOwl:hasOBONamespace>
        <oboInOwl:id>GAZ:00080610</oboInOwl:id>
        <rdfs:label>Landi Kotal Subdivision</rdfs:label>
    </owl:NamedIndividual>
    


    <!-- http://purl.obolibrary.org/obo/GAZ_00080611 -->

    <owl:NamedIndividual rdf:about="http://purl.obolibrary.org/obo/GAZ_00080611">
        <obo:RO_0001025 rdf:resource="http://purl.obolibrary.org/obo/GAZ_00018562"/>
        <obo:IAO_0000115>The mountain pass that links Pakistan and Afghanistan. As with many passes, the start and finish are ill-defined. Many definitions state that the Khyber Pass starts from near Jamrud, Pakistan (491 m), 15 km west of Peshawar and ends west of Torkham, Afghanistan, a winding road of 48 km which passes Fort Maude and Ali Masjid to reach a narrowest point of just 15 metre wide between canyon walls. The summit at Landi Kotal is followed by a steep decline to Michni Kandao, Landi Khana and the Afghan border at Torkham. Here the gradient becomes easier as the pass exits at Haft Chah opening onto the Dakka plain. The road/highway was built by the British in 1879 and the railway from Jamrud to Landi Khana was built over six years by Victor Bayley and completed in 1925.</obo:IAO_0000115>
        <oboInOwl:hasOBONamespace>GAZ</oboInOwl:hasOBONamespace>
        <oboInOwl:id>GAZ:00080611</oboInOwl:id>
        <rdfs:label>Khyber Pass</rdfs:label>
    </owl:NamedIndividual>
    


    <!-- http://purl.obolibrary.org/obo/GAZ_00080612 -->

    <owl:NamedIndividual rdf:about="http://purl.obolibrary.org/obo/GAZ_00080612">
        <obo:RO_0001025 rdf:resource="http://purl.obolibrary.org/obo/GAZ_00018556"/>
        <obo:IAO_0000115>A subdivision of North Waziristan Agency.</obo:IAO_0000115>
        <oboInOwl:hasOBONamespace>GAZ</oboInOwl:hasOBONamespace>
        <oboInOwl:id>GAZ:00080612</oboInOwl:id>
        <rdfs:label>Mir Ali Subdivision</rdfs:label>
    </owl:NamedIndividual>
    


    <!-- http://purl.obolibrary.org/obo/GAZ_00080613 -->

    <owl:NamedIndividual rdf:about="http://purl.obolibrary.org/obo/GAZ_00080613">
        <obo:RO_0001025 rdf:resource="http://purl.obolibrary.org/obo/GAZ_00080612"/>
        <obo:IAO_0000115>A Tehsil of the Mir Ali Subdivision, North Waziristan Agency.</obo:IAO_0000115>
        <oboInOwl:hasOBONamespace>GAZ</oboInOwl:hasOBONamespace>
        <oboInOwl:id>GAZ:00080613</oboInOwl:id>
        <rdfs:label>Mir Ali Tehsil</rdfs:label>
    </owl:NamedIndividual>
    


    <!-- http://purl.obolibrary.org/obo/GAZ_00080614 -->

    <owl:NamedIndividual rdf:about="http://purl.obolibrary.org/obo/GAZ_00080614">
        <obo:RO_0001025 rdf:resource="http://purl.obolibrary.org/obo/GAZ_00018556"/>
        <obo:IAO_0000115>A subdivision of North Waziristan Agency.</obo:IAO_0000115>
        <oboInOwl:hasOBONamespace>GAZ</oboInOwl:hasOBONamespace>
        <oboInOwl:id>GAZ:00080614</oboInOwl:id>
        <rdfs:label>Razmak Subdivision</rdfs:label>
    </owl:NamedIndividual>
    


    <!-- http://purl.obolibrary.org/obo/GAZ_00080615 -->

    <owl:NamedIndividual rdf:about="http://purl.obolibrary.org/obo/GAZ_00080615">
        <obo:RO_0001025 rdf:resource="http://purl.obolibrary.org/obo/GAZ_00080612"/>
        <obo:IAO_0000115>A Tehsil of the Mir Ali Subdivision, North Waziristan Agency.</obo:IAO_0000115>
        <oboInOwl:hasOBONamespace>GAZ</oboInOwl:hasOBONamespace>
        <oboInOwl:id>GAZ:00080615</oboInOwl:id>
        <rdfs:label>Shewa Tehsil</rdfs:label>
    </owl:NamedIndividual>
    


    <!-- http://purl.obolibrary.org/obo/GAZ_00080616 -->

    <owl:NamedIndividual rdf:about="http://purl.obolibrary.org/obo/GAZ_00080616">
        <obo:RO_0001025 rdf:resource="http://purl.obolibrary.org/obo/GAZ_00018556"/>
        <obo:IAO_0000115>A subdivision of North Waziristan Agency.</obo:IAO_0000115>
        <oboInOwl:hasOBONamespace>GAZ</oboInOwl:hasOBONamespace>
        <oboInOwl:id>GAZ:00080616</oboInOwl:id>
        <rdfs:label>Miran Shah Subdivision</rdfs:label>
    </owl:NamedIndividual>
    


    <!-- http://purl.obolibrary.org/obo/GAZ_00080617 -->

    <owl:NamedIndividual rdf:about="http://purl.obolibrary.org/obo/GAZ_00080617">
        <obo:RO_0001025 rdf:resource="http://purl.obolibrary.org/obo/GAZ_00080616"/>
        <obo:IAO_0000115>A Tehsil of the Miran Shah Subdivision, North Waziristan Agency.</obo:IAO_0000115>
        <oboInOwl:hasOBONamespace>GAZ</oboInOwl:hasOBONamespace>
        <oboInOwl:id>GAZ:00080617</oboInOwl:id>
        <rdfs:label>Miran Shah Tehsil</rdfs:label>
    </owl:NamedIndividual>
    


    <!-- http://purl.obolibrary.org/obo/GAZ_00080618 -->

    <owl:NamedIndividual rdf:about="http://purl.obolibrary.org/obo/GAZ_00080618">
        <obo:RO_0001025 rdf:resource="http://purl.obolibrary.org/obo/GAZ_00080616"/>
        <obo:IAO_0000115>A Tehsil of the Miran Shah Subdivision, North Waziristan Agency.</obo:IAO_0000115>
        <oboInOwl:hasOBONamespace>GAZ</oboInOwl:hasOBONamespace>
        <oboInOwl:id>GAZ:00080618</oboInOwl:id>
        <rdfs:label>Ghulam Khan Tehsil</rdfs:label>
    </owl:NamedIndividual>
    


    <!-- http://purl.obolibrary.org/obo/GAZ_00080619 -->

    <owl:NamedIndividual rdf:about="http://purl.obolibrary.org/obo/GAZ_00080619">
        <obo:RO_0001025 rdf:resource="http://purl.obolibrary.org/obo/GAZ_00080612"/>
        <obo:IAO_0000115>A Tehsil of the Mir Ali Subdivision, North Waziristan Agency.</obo:IAO_0000115>
        <oboInOwl:hasOBONamespace>GAZ</oboInOwl:hasOBONamespace>
        <oboInOwl:id>GAZ:00080619</oboInOwl:id>
        <rdfs:label>Spinwam Tehsil</rdfs:label>
    </owl:NamedIndividual>
    


    <!-- http://purl.obolibrary.org/obo/GAZ_00080620 -->

    <owl:NamedIndividual rdf:about="http://purl.obolibrary.org/obo/GAZ_00080620">
        <obo:RO_0001025 rdf:resource="http://purl.obolibrary.org/obo/GAZ_00080616"/>
        <obo:IAO_0000115>A Tehsil of the Miran Shah Subdivision, North Waziristan Agency.</obo:IAO_0000115>
        <oboInOwl:hasOBONamespace>GAZ</oboInOwl:hasOBONamespace>
        <oboInOwl:id>GAZ:00080620</oboInOwl:id>
        <rdfs:label>Datta Khel Tehsil</rdfs:label>
    </owl:NamedIndividual>
    


    <!-- http://purl.obolibrary.org/obo/GAZ_00080621 -->

    <owl:NamedIndividual rdf:about="http://purl.obolibrary.org/obo/GAZ_00080621">
        <obo:RO_0001025 rdf:resource="http://purl.obolibrary.org/obo/GAZ_00080614"/>
        <obo:IAO_0000115>A Tehsil of the Razmak Subdivision, North Waziristan Agency.</obo:IAO_0000115>
        <oboInOwl:hasOBONamespace>GAZ</oboInOwl:hasOBONamespace>
        <oboInOwl:id>GAZ:00080621</oboInOwl:id>
        <rdfs:label>Dossali Tehsil</rdfs:label>
    </owl:NamedIndividual>
    


    <!-- http://purl.obolibrary.org/obo/GAZ_00080622 -->

    <owl:NamedIndividual rdf:about="http://purl.obolibrary.org/obo/GAZ_00080622">
        <obo:RO_0001025 rdf:resource="http://purl.obolibrary.org/obo/GAZ_00080614"/>
        <obo:IAO_0000115>A Tehsil of the Razmak Subdivision, North Waziristan Agency.</obo:IAO_0000115>
        <oboInOwl:hasOBONamespace>GAZ</oboInOwl:hasOBONamespace>
        <oboInOwl:id>GAZ:00080622</oboInOwl:id>
        <rdfs:label>Razmak Tehsil</rdfs:label>
    </owl:NamedIndividual>
    


    <!-- http://purl.obolibrary.org/obo/GAZ_00080623 -->

    <owl:NamedIndividual rdf:about="http://purl.obolibrary.org/obo/GAZ_00080623">
        <obo:RO_0001025 rdf:resource="http://purl.obolibrary.org/obo/GAZ_00080614"/>
        <obo:IAO_0000115>A Tehsil of the Razmak Subdivision, North Waziristan Agency.</obo:IAO_0000115>
        <oboInOwl:hasOBONamespace>GAZ</oboInOwl:hasOBONamespace>
        <oboInOwl:id>GAZ:00080623</oboInOwl:id>
        <rdfs:label>Garyum Tehsil</rdfs:label>
    </owl:NamedIndividual>
    


    <!-- http://purl.obolibrary.org/obo/GAZ_00080624 -->

    <owl:NamedIndividual rdf:about="http://purl.obolibrary.org/obo/GAZ_00080624">
        <obo:RO_0001025 rdf:resource="http://purl.obolibrary.org/obo/GAZ_00018564"/>
        <obo:IAO_0000115>A Tehsil of the Mohmand Agency.</obo:IAO_0000115>
        <oboInOwl:hasOBONamespace>GAZ</oboInOwl:hasOBONamespace>
        <oboInOwl:id>GAZ:00080624</oboInOwl:id>
        <rdfs:label>Pindiali Tehsil</rdfs:label>
    </owl:NamedIndividual>
    


    <!-- http://purl.obolibrary.org/obo/GAZ_00080625 -->

    <owl:NamedIndividual rdf:about="http://purl.obolibrary.org/obo/GAZ_00080625">
        <obo:RO_0001025 rdf:resource="http://purl.obolibrary.org/obo/GAZ_00018564"/>
        <obo:IAO_0000115>A Tehsil of the Mohmand Agency.</obo:IAO_0000115>
        <oboInOwl:hasOBONamespace>GAZ</oboInOwl:hasOBONamespace>
        <oboInOwl:id>GAZ:00080625</oboInOwl:id>
        <rdfs:label>Yake Ghund Tehsil</rdfs:label>
    </owl:NamedIndividual>
    


    <!-- http://purl.obolibrary.org/obo/GAZ_00080626 -->

    <owl:NamedIndividual rdf:about="http://purl.obolibrary.org/obo/GAZ_00080626">
        <obo:RO_0001025 rdf:resource="http://purl.obolibrary.org/obo/GAZ_00018564"/>
        <obo:IAO_0000115>A Tehsil of the Mohmand Agency.</obo:IAO_0000115>
        <oboInOwl:hasOBONamespace>GAZ</oboInOwl:hasOBONamespace>
        <oboInOwl:id>GAZ:00080626</oboInOwl:id>
        <rdfs:label>Upper Mohmand Tehsil</rdfs:label>
    </owl:NamedIndividual>
    


    <!-- http://purl.obolibrary.org/obo/GAZ_00080627 -->

    <owl:NamedIndividual rdf:about="http://purl.obolibrary.org/obo/GAZ_00080627">
        <obo:RO_0001025 rdf:resource="http://purl.obolibrary.org/obo/GAZ_00018564"/>
        <obo:IAO_0000115>A Tehsil of the Mohmand Agency.</obo:IAO_0000115>
        <oboInOwl:hasOBONamespace>GAZ</oboInOwl:hasOBONamespace>
        <oboInOwl:id>GAZ:00080627</oboInOwl:id>
        <rdfs:label>Utman Khel (Ambar) Tehsil</rdfs:label>
    </owl:NamedIndividual>
    


    <!-- http://purl.obolibrary.org/obo/GAZ_00080628 -->

    <owl:NamedIndividual rdf:about="http://purl.obolibrary.org/obo/GAZ_00080628">
        <obo:RO_0001025 rdf:resource="http://purl.obolibrary.org/obo/GAZ_00018564"/>
        <obo:IAO_0000115>A Tehsil of the Mohmand Agency.</obo:IAO_0000115>
        <oboInOwl:hasOBONamespace>GAZ</oboInOwl:hasOBONamespace>
        <oboInOwl:id>GAZ:00080628</oboInOwl:id>
        <rdfs:label>Safi Tehsil</rdfs:label>
    </owl:NamedIndividual>
    


    <!-- http://purl.obolibrary.org/obo/GAZ_00080629 -->

    <owl:NamedIndividual rdf:about="http://purl.obolibrary.org/obo/GAZ_00080629">
        <obo:RO_0001025 rdf:resource="http://purl.obolibrary.org/obo/GAZ_00018564"/>
        <obo:IAO_0000115>A Tehsil of the Mohmand Agency.</obo:IAO_0000115>
        <oboInOwl:hasOBONamespace>GAZ</oboInOwl:hasOBONamespace>
        <oboInOwl:id>GAZ:00080629</oboInOwl:id>
        <rdfs:label>Halimzai Tehsil</rdfs:label>
    </owl:NamedIndividual>
    


    <!-- http://purl.obolibrary.org/obo/GAZ_00080630 -->

    <owl:NamedIndividual rdf:about="http://purl.obolibrary.org/obo/GAZ_00080630">
        <obo:RO_0001025 rdf:resource="http://purl.obolibrary.org/obo/GAZ_00018564"/>
        <obo:IAO_0000115>A Tehsil of the Mohmand Agency.</obo:IAO_0000115>
        <oboInOwl:hasOBONamespace>GAZ</oboInOwl:hasOBONamespace>
        <oboInOwl:id>GAZ:00080630</oboInOwl:id>
        <rdfs:label>Pringhar Tehsil</rdfs:label>
    </owl:NamedIndividual>
    


    <!-- http://purl.obolibrary.org/obo/GAZ_00080631 -->

    <owl:NamedIndividual rdf:about="http://purl.obolibrary.org/obo/GAZ_00080631">
        <obo:RO_0001025 rdf:resource="http://purl.obolibrary.org/obo/GAZ_00018560"/>
        <obo:IAO_0000115>A Tehsil of the Kurram Agency.</obo:IAO_0000115>
        <oboInOwl:hasOBONamespace>GAZ</oboInOwl:hasOBONamespace>
        <oboInOwl:id>GAZ:00080631</oboInOwl:id>
        <rdfs:label>Upper Kurram Tehsil</rdfs:label>
    </owl:NamedIndividual>
    


    <!-- http://purl.obolibrary.org/obo/GAZ_00080632 -->

    <owl:NamedIndividual rdf:about="http://purl.obolibrary.org/obo/GAZ_00080632">
        <obo:RO_0001025 rdf:resource="http://purl.obolibrary.org/obo/GAZ_00018560"/>
        <obo:IAO_0000115>A Tehsil of the Kurram Agency.</obo:IAO_0000115>
        <oboInOwl:hasOBONamespace>GAZ</oboInOwl:hasOBONamespace>
        <oboInOwl:id>GAZ:00080632</oboInOwl:id>
        <rdfs:label>Lower Kurram Tehsil</rdfs:label>
    </owl:NamedIndividual>
    


    <!-- http://purl.obolibrary.org/obo/GAZ_00080633 -->

    <owl:NamedIndividual rdf:about="http://purl.obolibrary.org/obo/GAZ_00080633">
        <obo:RO_0001025 rdf:resource="http://purl.obolibrary.org/obo/GAZ_00018560"/>
        <obo:IAO_0000115>A Tehsil of the Kurram Agency.</obo:IAO_0000115>
        <oboInOwl:hasOBONamespace>GAZ</oboInOwl:hasOBONamespace>
        <oboInOwl:id>GAZ:00080633</oboInOwl:id>
        <rdfs:label>Kurram F.R. Tehsil</rdfs:label>
    </owl:NamedIndividual>
    


    <!-- http://purl.obolibrary.org/obo/GAZ_00080634 -->

    <owl:NamedIndividual rdf:about="http://purl.obolibrary.org/obo/GAZ_00080634">
        <obo:RO_0001025 rdf:resource="http://purl.obolibrary.org/obo/GAZ_00018563"/>
        <obo:IAO_0000115>A Tehsil in the Orakzai Agency.</obo:IAO_0000115>
        <oboInOwl:hasOBONamespace>GAZ</oboInOwl:hasOBONamespace>
        <oboInOwl:id>GAZ:00080634</oboInOwl:id>
        <rdfs:label>Lower Orakzai Tehsil</rdfs:label>
    </owl:NamedIndividual>
    


    <!-- http://purl.obolibrary.org/obo/GAZ_00080635 -->

    <owl:NamedIndividual rdf:about="http://purl.obolibrary.org/obo/GAZ_00080635">
        <obo:RO_0001025 rdf:resource="http://purl.obolibrary.org/obo/GAZ_00018563"/>
        <obo:IAO_0000115>A Tehsil in the Orakzai Agency.</obo:IAO_0000115>
        <oboInOwl:hasOBONamespace>GAZ</oboInOwl:hasOBONamespace>
        <oboInOwl:id>GAZ:00080635</oboInOwl:id>
        <rdfs:label>Central Orakzai Tehsil</rdfs:label>
    </owl:NamedIndividual>
    


    <!-- http://purl.obolibrary.org/obo/GAZ_00080636 -->

    <owl:NamedIndividual rdf:about="http://purl.obolibrary.org/obo/GAZ_00080636">
        <obo:RO_0001025 rdf:resource="http://purl.obolibrary.org/obo/GAZ_00018563"/>
        <obo:IAO_0000115>A Tehsil in the Orakzai Agency.</obo:IAO_0000115>
        <oboInOwl:hasOBONamespace>GAZ</oboInOwl:hasOBONamespace>
        <oboInOwl:id>GAZ:00080636</oboInOwl:id>
        <rdfs:label>Ismailzai Tehsil</rdfs:label>
    </owl:NamedIndividual>
    


    <!-- http://purl.obolibrary.org/obo/GAZ_00080637 -->

    <owl:NamedIndividual rdf:about="http://purl.obolibrary.org/obo/GAZ_00080637">
        <obo:RO_0001025 rdf:resource="http://purl.obolibrary.org/obo/GAZ_00018563"/>
        <obo:IAO_0000115>A Tehsil in the Orakzai Agency.</obo:IAO_0000115>
        <oboInOwl:hasOBONamespace>GAZ</oboInOwl:hasOBONamespace>
        <oboInOwl:id>GAZ:00080637</oboInOwl:id>
        <rdfs:label>Upper Orakzai Tehsil</rdfs:label>
    </owl:NamedIndividual>
    


    <!-- http://purl.obolibrary.org/obo/GAZ_00080638 -->

    <owl:NamedIndividual rdf:about="http://purl.obolibrary.org/obo/GAZ_00080638">
        <obo:RO_0001025 rdf:resource="http://purl.obolibrary.org/obo/GAZ_00018561"/>
        <obo:IAO_0000115>A Tehsil of the Bajaur Agency.</obo:IAO_0000115>
        <oboInOwl:hasOBONamespace>GAZ</oboInOwl:hasOBONamespace>
        <oboInOwl:id>GAZ:00080638</oboInOwl:id>
        <rdfs:label>Charmang Tehsil</rdfs:label>
    </owl:NamedIndividual>
    


    <!-- http://purl.obolibrary.org/obo/GAZ_00080639 -->

    <owl:NamedIndividual rdf:about="http://purl.obolibrary.org/obo/GAZ_00080639">
        <obo:RO_0001025 rdf:resource="http://purl.obolibrary.org/obo/GAZ_00018561"/>
        <obo:IAO_0000115>A Tehsil of the Bajaur Agency.</obo:IAO_0000115>
        <oboInOwl:hasOBONamespace>GAZ</oboInOwl:hasOBONamespace>
        <oboInOwl:id>GAZ:00080639</oboInOwl:id>
        <rdfs:label>Barang Tehsil</rdfs:label>
    </owl:NamedIndividual>
    


    <!-- http://purl.obolibrary.org/obo/GAZ_00080640 -->

    <owl:NamedIndividual rdf:about="http://purl.obolibrary.org/obo/GAZ_00080640">
        <obo:RO_0001025 rdf:resource="http://purl.obolibrary.org/obo/GAZ_00018561"/>
        <obo:IAO_0000115>A Tehsil of the Bajaur Agency.</obo:IAO_0000115>
        <oboInOwl:hasOBONamespace>GAZ</oboInOwl:hasOBONamespace>
        <oboInOwl:id>GAZ:00080640</oboInOwl:id>
        <rdfs:label>Nawagai Tehsil</rdfs:label>
    </owl:NamedIndividual>
    


    <!-- http://purl.obolibrary.org/obo/GAZ_00080641 -->

    <owl:NamedIndividual rdf:about="http://purl.obolibrary.org/obo/GAZ_00080641">
        <obo:RO_0001025 rdf:resource="http://purl.obolibrary.org/obo/GAZ_00018561"/>
        <obo:IAO_0000115>A Tehsil of the Bajaur Agency.</obo:IAO_0000115>
        <oboInOwl:hasOBONamespace>GAZ</oboInOwl:hasOBONamespace>
        <oboInOwl:id>GAZ:00080641</oboInOwl:id>
        <rdfs:label>Mamund Tehsil</rdfs:label>
    </owl:NamedIndividual>
    


    <!-- http://purl.obolibrary.org/obo/GAZ_00080642 -->

    <owl:NamedIndividual rdf:about="http://purl.obolibrary.org/obo/GAZ_00080642">
        <obo:RO_0001025 rdf:resource="http://purl.obolibrary.org/obo/GAZ_00018561"/>
        <obo:IAO_0000115>A Tehsil of the Bajaur Agency.</obo:IAO_0000115>
        <oboInOwl:hasOBONamespace>GAZ</oboInOwl:hasOBONamespace>
        <oboInOwl:id>GAZ:00080642</oboInOwl:id>
        <rdfs:label>Khar Bajaur Tehsil</rdfs:label>
    </owl:NamedIndividual>
    


    <!-- http://purl.obolibrary.org/obo/GAZ_00080643 -->

    <owl:NamedIndividual rdf:about="http://purl.obolibrary.org/obo/GAZ_00080643">
        <obo:RO_0001025 rdf:resource="http://purl.obolibrary.org/obo/GAZ_00018561"/>
        <obo:IAO_0000115>A Tehsil of the Bajaur Agency.</obo:IAO_0000115>
        <oboInOwl:hasOBONamespace>GAZ</oboInOwl:hasOBONamespace>
        <oboInOwl:id>GAZ:00080643</oboInOwl:id>
        <rdfs:label>Salarzai Tehsil</rdfs:label>
    </owl:NamedIndividual>
    


    <!-- http://purl.obolibrary.org/obo/GAZ_00080644 -->

    <owl:NamedIndividual rdf:about="http://purl.obolibrary.org/obo/GAZ_00080644">
        <obo:RO_0001025 rdf:resource="http://purl.obolibrary.org/obo/GAZ_00018561"/>
        <obo:IAO_0000115>A Tehsil of the Bajaur Agency.</obo:IAO_0000115>
        <oboInOwl:hasOBONamespace>GAZ</oboInOwl:hasOBONamespace>
        <oboInOwl:id>GAZ:00080644</oboInOwl:id>
        <rdfs:label>Utmankhel (Qzafi) Tehsil</rdfs:label>
    </owl:NamedIndividual>
    


    <!-- http://purl.obolibrary.org/obo/GAZ_00080645 -->

    <owl:NamedIndividual rdf:about="http://purl.obolibrary.org/obo/GAZ_00080645">
        <obo:RO_0001025 rdf:resource="http://purl.obolibrary.org/obo/GAZ_00018580"/>
        <obo:IAO_0000115>A Tehsil in Skardu District.</obo:IAO_0000115>
        <oboInOwl:hasOBONamespace>GAZ</oboInOwl:hasOBONamespace>
        <oboInOwl:id>GAZ:00080645</oboInOwl:id>
        <rdfs:label>Rondu Tehsil</rdfs:label>
    </owl:NamedIndividual>
    


    <!-- http://purl.obolibrary.org/obo/GAZ_00080646 -->

    <owl:NamedIndividual rdf:about="http://purl.obolibrary.org/obo/GAZ_00080646">
        <obo:RO_0001025 rdf:resource="http://purl.obolibrary.org/obo/GAZ_00018580"/>
        <obo:IAO_0000115>A Tehsil in Skardu District.</obo:IAO_0000115>
        <oboInOwl:hasOBONamespace>GAZ</oboInOwl:hasOBONamespace>
        <oboInOwl:id>GAZ:00080646</oboInOwl:id>
        <rdfs:label>Gultari Tehsil</rdfs:label>
    </owl:NamedIndividual>
    


    <!-- http://purl.obolibrary.org/obo/GAZ_00080647 -->

    <owl:NamedIndividual rdf:about="http://purl.obolibrary.org/obo/GAZ_00080647">
        <obo:RO_0001025 rdf:resource="http://purl.obolibrary.org/obo/GAZ_00018580"/>
        <obo:IAO_0000115>A Tehsil in Skardu District.</obo:IAO_0000115>
        <oboInOwl:hasOBONamespace>GAZ</oboInOwl:hasOBONamespace>
        <oboInOwl:id>GAZ:00080647</oboInOwl:id>
        <rdfs:label>Kharmang Tehsil</rdfs:label>
    </owl:NamedIndividual>
    


    <!-- http://purl.obolibrary.org/obo/GAZ_00080648 -->

    <owl:NamedIndividual rdf:about="http://purl.obolibrary.org/obo/GAZ_00080648">
        <obo:RO_0001025 rdf:resource="http://purl.obolibrary.org/obo/GAZ_00018580"/>
        <obo:IAO_0000115>A Tehsil in Skardu District.</obo:IAO_0000115>
        <oboInOwl:hasOBONamespace>GAZ</oboInOwl:hasOBONamespace>
        <oboInOwl:id>GAZ:00080648</oboInOwl:id>
        <rdfs:label>Shigar Tehsil</rdfs:label>
    </owl:NamedIndividual>
    


    <!-- http://purl.obolibrary.org/obo/GAZ_00080649 -->

    <owl:NamedIndividual rdf:about="http://purl.obolibrary.org/obo/GAZ_00080649">
        <obo:RO_0001025 rdf:resource="http://purl.obolibrary.org/obo/GAZ_00018581"/>
        <obo:IAO_0000115>A Tehsil in Ghanche District.</obo:IAO_0000115>
        <oboInOwl:hasOBONamespace>GAZ</oboInOwl:hasOBONamespace>
        <oboInOwl:id>GAZ:00080649</oboInOwl:id>
        <rdfs:label>Khaplu Tehsil</rdfs:label>
    </owl:NamedIndividual>
    


    <!-- http://purl.obolibrary.org/obo/GAZ_00080650 -->

    <owl:NamedIndividual rdf:about="http://purl.obolibrary.org/obo/GAZ_00080650">
        <obo:RO_0001025 rdf:resource="http://purl.obolibrary.org/obo/GAZ_00018581"/>
        <obo:IAO_0000115>A Tehsil in Ghanche District.</obo:IAO_0000115>
        <oboInOwl:hasOBONamespace>GAZ</oboInOwl:hasOBONamespace>
        <oboInOwl:id>GAZ:00080650</oboInOwl:id>
        <rdfs:label>Masherbrum Tehsil</rdfs:label>
    </owl:NamedIndividual>
    


    <!-- http://purl.obolibrary.org/obo/GAZ_00080651 -->

    <owl:NamedIndividual rdf:about="http://purl.obolibrary.org/obo/GAZ_00080651">
        <obo:RO_0001025 rdf:resource="http://purl.obolibrary.org/obo/GAZ_00018578"/>
        <obo:IAO_0000115>The Tehsil of Astore District.</obo:IAO_0000115>
        <oboInOwl:hasOBONamespace>GAZ</oboInOwl:hasOBONamespace>
        <oboInOwl:id>GAZ:00080651</oboInOwl:id>
        <rdfs:label>Astore Tehsil</rdfs:label>
    </owl:NamedIndividual>
    


    <!-- http://purl.obolibrary.org/obo/GAZ_00080652 -->

    <owl:NamedIndividual rdf:about="http://purl.obolibrary.org/obo/GAZ_00080652">
        <obo:RO_0001025 rdf:resource="http://purl.obolibrary.org/obo/GAZ_00018583"/>
        <obo:IAO_0000115>A Tehsil in Giglit District.</obo:IAO_0000115>
        <oboInOwl:hasOBONamespace>GAZ</oboInOwl:hasOBONamespace>
        <oboInOwl:id>GAZ:00080652</oboInOwl:id>
        <rdfs:label>Allabad Tehsil</rdfs:label>
    </owl:NamedIndividual>
    


    <!-- http://purl.obolibrary.org/obo/GAZ_00080653 -->

    <owl:NamedIndividual rdf:about="http://purl.obolibrary.org/obo/GAZ_00080653">
        <obo:RO_0001025 rdf:resource="http://purl.obolibrary.org/obo/GAZ_00018583"/>
        <obo:IAO_0000115>A Tehsil in Giglit District.</obo:IAO_0000115>
        <oboInOwl:hasOBONamespace>GAZ</oboInOwl:hasOBONamespace>
        <oboInOwl:id>GAZ:00080653</oboInOwl:id>
        <rdfs:label>Nagar-I Tehsil</rdfs:label>
    </owl:NamedIndividual>
    


    <!-- http://purl.obolibrary.org/obo/GAZ_00080654 -->

    <owl:NamedIndividual rdf:about="http://purl.obolibrary.org/obo/GAZ_00080654">
        <obo:RO_0001025 rdf:resource="http://purl.obolibrary.org/obo/GAZ_00018583"/>
        <obo:IAO_0000115>A Tehsil in Giglit District.</obo:IAO_0000115>
        <oboInOwl:hasOBONamespace>GAZ</oboInOwl:hasOBONamespace>
        <oboInOwl:id>GAZ:00080654</oboInOwl:id>
        <rdfs:label>Giglit Tehsil</rdfs:label>
    </owl:NamedIndividual>
    


    <!-- http://purl.obolibrary.org/obo/GAZ_00080655 -->

    <owl:NamedIndividual rdf:about="http://purl.obolibrary.org/obo/GAZ_00080655">
        <obo:RO_0001025 rdf:resource="http://purl.obolibrary.org/obo/GAZ_00018583"/>
        <obo:IAO_0000115>A Tehsil in Giglit District.</obo:IAO_0000115>
        <oboInOwl:hasOBONamespace>GAZ</oboInOwl:hasOBONamespace>
        <oboInOwl:id>GAZ:00080655</oboInOwl:id>
        <rdfs:label>Nagar-II Tehsil</rdfs:label>
    </owl:NamedIndividual>
    


    <!-- http://purl.obolibrary.org/obo/GAZ_00080656 -->

    <owl:NamedIndividual rdf:about="http://purl.obolibrary.org/obo/GAZ_00080656">
        <obo:RO_0001025 rdf:resource="http://purl.obolibrary.org/obo/GAZ_00018582"/>
        <obo:IAO_0000115>A Tehsil in Diamer District.</obo:IAO_0000115>
        <oboInOwl:hasOBONamespace>GAZ</oboInOwl:hasOBONamespace>
        <oboInOwl:id>GAZ:00080656</oboInOwl:id>
        <rdfs:label>Darel/Tangir Tehsil</rdfs:label>
    </owl:NamedIndividual>
    


    <!-- http://purl.obolibrary.org/obo/GAZ_00080657 -->

    <owl:NamedIndividual rdf:about="http://purl.obolibrary.org/obo/GAZ_00080657">
        <obo:RO_0001025 rdf:resource="http://purl.obolibrary.org/obo/GAZ_00018582"/>
        <obo:IAO_0000115>A Tehsil in Diamer District.</obo:IAO_0000115>
        <oboInOwl:hasOBONamespace>GAZ</oboInOwl:hasOBONamespace>
        <oboInOwl:id>GAZ:00080657</oboInOwl:id>
        <rdfs:label>Chilas Tehsil</rdfs:label>
    </owl:NamedIndividual>
    


    <!-- http://purl.obolibrary.org/obo/GAZ_00080658 -->

    <owl:NamedIndividual rdf:about="http://purl.obolibrary.org/obo/GAZ_00080658">
        <obo:RO_0001025 rdf:resource="http://purl.obolibrary.org/obo/GAZ_00018576"/>
        <obo:IAO_0000115>A Tehsil in Ghizer District.</obo:IAO_0000115>
        <oboInOwl:hasOBONamespace>GAZ</oboInOwl:hasOBONamespace>
        <oboInOwl:id>GAZ:00080658</oboInOwl:id>
        <rdfs:label>Yasin Tehsil</rdfs:label>
    </owl:NamedIndividual>
    


    <!-- http://purl.obolibrary.org/obo/GAZ_00080659 -->

    <owl:NamedIndividual rdf:about="http://purl.obolibrary.org/obo/GAZ_00080659">
        <obo:RO_0001025 rdf:resource="http://purl.obolibrary.org/obo/GAZ_00018576"/>
        <obo:IAO_0000115>A Tehsil in Ghizer District.</obo:IAO_0000115>
        <oboInOwl:hasOBONamespace>GAZ</oboInOwl:hasOBONamespace>
        <oboInOwl:id>GAZ:00080659</oboInOwl:id>
        <rdfs:label>Puniyal Tehsil</rdfs:label>
    </owl:NamedIndividual>
    


    <!-- http://purl.obolibrary.org/obo/GAZ_00080660 -->

    <owl:NamedIndividual rdf:about="http://purl.obolibrary.org/obo/GAZ_00080660">
        <obo:RO_0001025 rdf:resource="http://purl.obolibrary.org/obo/GAZ_00018576"/>
        <obo:IAO_0000115>A Tehsil in Ghizer District.</obo:IAO_0000115>
        <oboInOwl:hasOBONamespace>GAZ</oboInOwl:hasOBONamespace>
        <oboInOwl:id>GAZ:00080660</oboInOwl:id>
        <rdfs:label>Ishkomen Tehsil</rdfs:label>
    </owl:NamedIndividual>
    


    <!-- http://purl.obolibrary.org/obo/GAZ_00080661 -->

    <owl:NamedIndividual rdf:about="http://purl.obolibrary.org/obo/GAZ_00080661">
        <obo:RO_0001025 rdf:resource="http://purl.obolibrary.org/obo/GAZ_00018576"/>
        <obo:IAO_0000115>A Tehsil in Ghizer District.</obo:IAO_0000115>
        <oboInOwl:hasOBONamespace>GAZ</oboInOwl:hasOBONamespace>
        <oboInOwl:id>GAZ:00080661</oboInOwl:id>
        <rdfs:label>Gupis Tehsil</rdfs:label>
    </owl:NamedIndividual>
    


    <!-- http://purl.obolibrary.org/obo/GAZ_00080662 -->

    <owl:NamedIndividual rdf:about="http://purl.obolibrary.org/obo/GAZ_00080662">
        <obo:RO_0001025 rdf:resource="http://purl.obolibrary.org/obo/GAZ_00018583"/>
        <obo:IAO_0000115>A lake in Gilgit District.</obo:IAO_0000115>
        <oboInOwl:hasOBONamespace>GAZ</oboInOwl:hasOBONamespace>
        <oboInOwl:id>GAZ:00080662</oboInOwl:id>
        <rdfs:label>Borit Lake</rdfs:label>
    </owl:NamedIndividual>
    


    <!-- http://purl.obolibrary.org/obo/GAZ_00129987 -->

    <owl:NamedIndividual rdf:about="http://purl.obolibrary.org/obo/GAZ_00129987">
        <obo:RO_0001025 rdf:resource="http://purl.obolibrary.org/obo/GAZ_00011784"/>
        <obo:IAO_0000115>A protected area. It consists of the northern part of the massif of Mount Everest in the southwest corner of the Tibet Autonomous Region in the border region between the Tibetan, China and Nepal biogeographical realms. It extends from the border with Nepal in the south, to the watershed between the Yaluzangbu River and the southern regions of Tibet in the north.</obo:IAO_0000115>
        <oboInOwl:hasOBONamespace>GAZ</oboInOwl:hasOBONamespace>
        <oboInOwl:id>GAZ:00129987</oboInOwl:id>
        <rdfs:label>Qomolangma National Nature Reserve</rdfs:label>
    </owl:NamedIndividual>
    


    <!-- http://purl.obolibrary.org/obo/GAZ_00143916 -->

    <owl:NamedIndividual rdf:about="http://purl.obolibrary.org/obo/GAZ_00143916">
        <obo:RO_0001025 rdf:resource="http://purl.obolibrary.org/obo/GAZ_00004988"/>
        <obo:IAO_0000115>A large glacier in the Pamir Mountains of central Tajikistan. The glacier follows a generally northward path to the east of the 6,595 m Garmo Peak. The glacier begins at an elevation of 6,200 m above sea level, and eventually melts and empties into the Balandkiik River near the border with Kyrgyzstan at an elevation of 2,909 m. Its waters eventually feed into the Muksu, Vakhsh, and Amu Darya rivers.</obo:IAO_0000115>
        <oboInOwl:hasOBONamespace>GAZ</oboInOwl:hasOBONamespace>
        <oboInOwl:id>GAZ:00143916</oboInOwl:id>
        <rdfs:label>Fedchenko Glacier</rdfs:label>
    </owl:NamedIndividual>
    


    <!-- http://purl.obolibrary.org/obo/GAZ_00143917 -->

    <owl:NamedIndividual rdf:about="http://purl.obolibrary.org/obo/GAZ_00143917">
        <obo:RO_0001025 rdf:resource="http://purl.obolibrary.org/obo/GAZ_00004988"/>
        <obo:IAO_0000115>A glacier in the Pamir Mountains, near Qullai Revolutsiya, Gorno-Badakhshan, central Tajikistan.</obo:IAO_0000115>
        <oboInOwl:hasOBONamespace>GAZ</oboInOwl:hasOBONamespace>
        <oboInOwl:id>GAZ:00143917</oboInOwl:id>
        <rdfs:label>Russian Geographical Society Glacier</rdfs:label>
    </owl:NamedIndividual>
    


    <!-- http://purl.obolibrary.org/obo/GAZ_00144828 -->

    <owl:NamedIndividual rdf:about="http://purl.obolibrary.org/obo/GAZ_00144828">
        <obo:RO_0001025 rdf:resource="http://purl.obolibrary.org/obo/GAZ_00004988"/>
        <obo:IAO_0000115>A mountain range in Central Asia, in the western part of the Pamir-Alay system, stretching over 200 km in the general east-west direction across the territory of Tajikistan and Uzbekistan. The Gissar Range lies south of the Zeravshan Range, extending north of Dushanbe through Tajikistan&apos;s Gissar District and reaching Uzbekistan at the north tip of Surkhandarya Province.</obo:IAO_0000115>
        <oboInOwl:hasOBONamespace>GAZ</oboInOwl:hasOBONamespace>
        <oboInOwl:id>GAZ:00144828</oboInOwl:id>
        <rdfs:label>Gissar Range</rdfs:label>
    </owl:NamedIndividual>
    


    <!-- http://purl.obolibrary.org/obo/GAZ_00144830 -->

    <owl:NamedIndividual rdf:about="http://purl.obolibrary.org/obo/GAZ_00144830">
        <obo:RO_0001025 rdf:resource="http://purl.obolibrary.org/obo/GAZ_00004988"/>
        <obo:IAO_0000115>A mountain range that rises to the south of the Zeravshan River. The range extends over 370 km in the east-west direction along the south of Sughd Province in Tajikistan, reaching the highest point of 5,489 m (Chimtarga peak) in its central part. South-west of Penjikent the range crosses from Tajikistan into Uzbekistan, where it continues at decreasing elevations (1,500-2,000 m) along the internal border between Samarkand and Surkhandarya provinces, until it blends into the desert south-west of Samarkand.</obo:IAO_0000115>
        <oboInOwl:hasOBONamespace>GAZ</oboInOwl:hasOBONamespace>
        <oboInOwl:id>GAZ:00144830</oboInOwl:id>
        <rdfs:label>Zeravshan Range</rdfs:label>
    </owl:NamedIndividual>
    


    <!-- http://purl.obolibrary.org/obo/GAZ_00145474 -->

    <owl:NamedIndividual rdf:about="http://purl.obolibrary.org/obo/GAZ_00145474">
        <obo:IAO_0000115>A tidal reek in the Kutch region of the Indian State of Gujarat. It lies in the Rann of Kutch marshland near the Sir Creek, which is disputed between India and Pakistan.</obo:IAO_0000115>
        <oboInOwl:hasOBONamespace>GAZ</oboInOwl:hasOBONamespace>
        <oboInOwl:id>GAZ:00145474</oboInOwl:id>
        <rdfs:label>Kori Creek</rdfs:label>
    </owl:NamedIndividual>
    


    <!-- http://purl.obolibrary.org/obo/GAZ_00145478 -->

    <owl:NamedIndividual rdf:about="http://purl.obolibrary.org/obo/GAZ_00145478">
        <obo:IAO_0000115>A 96 km strip of water disputed between India and Pakistan in the Rann of Kutch marshlands. The creek, which opens up into the Arabian Sea, divides the Kutch region of the Indian State of Gujarat with the Sindh province of Pakistan.</obo:IAO_0000115>
        <oboInOwl:hasOBONamespace>GAZ</oboInOwl:hasOBONamespace>
        <oboInOwl:id>GAZ:00145478</oboInOwl:id>
        <rdfs:label>Sir Creek</rdfs:label>
    </owl:NamedIndividual>
    


    <!-- http://purl.obolibrary.org/obo/GAZ_00147860 -->

    <owl:NamedIndividual rdf:about="http://purl.obolibrary.org/obo/GAZ_00147860">
        <obo:RO_0001025 rdf:resource="http://purl.obolibrary.org/obo/GAZ_00005246"/>
        <obo:IAO_0000115>A delta that is formed where the Indus River flows into the Arabian Sea in Pakistan. A Ramsar Site. A Ramsar Site.</obo:IAO_0000115>
        <oboInOwl:hasOBONamespace>GAZ</oboInOwl:hasOBONamespace>
        <oboInOwl:id>GAZ:00147860</oboInOwl:id>
        <rdfs:label>Indus River Delta</rdfs:label>
    </owl:NamedIndividual>
    


    <!-- http://purl.obolibrary.org/obo/GAZ_00148807 -->

    <owl:NamedIndividual rdf:about="http://purl.obolibrary.org/obo/GAZ_00148807">
        <obo:IAO_0000115>The longest of the five rivers that flow through the historic crossroad region of Punjab in northern India and Pakistan. It is located north of the Vindhya Range, south of the Hindu Kush segment of the Himalayas, and east of the Central Sulaiman Range in Pakistan. It is the easternmost tributary of the Indus River. Its source is at Lake Rakshastal in Tibet near Mount Kailas, and it flows generally west and southwest. It waters the ancient and historically important region of Greater Punjab. The region to its south and east is arid, and is known as the Great Indian Desert or Thar Desert. Sutlej joins with the Beas River in the State of Punjab, India, and continues southwest into Pakistan to unite with the Chenab river, forming the Panjnad River south of ancient Multan. The Panjnad joins the Indus river at Mithankot. Indus then flows through a gorge near Sukkur, flows through the fertile plains region of Sindh, and terminates in the Arabian Sea near the port city of Karachi in Pakistan.</obo:IAO_0000115>
        <oboInOwl:hasOBONamespace>GAZ</oboInOwl:hasOBONamespace>
        <oboInOwl:id>GAZ:00148807</oboInOwl:id>
        <rdfs:label>Sutlej River</rdfs:label>
    </owl:NamedIndividual>
    


    <!-- http://purl.obolibrary.org/obo/GAZ_00148844 -->

    <owl:NamedIndividual rdf:about="http://purl.obolibrary.org/obo/GAZ_00148844">
        <obo:IAO_0000115>The longest river in Afghanistan and the primarily watershed for the endorheic Sistan Basin. The Helmand river stretches for 1,150 km. It rises in the Hindu Kush mountains, about 80 km west of Kabul, passing north of the Unai Pass. It crosses south-west through the desert of Dashti Margo, to the Seistan marshes and the Hamun-i-Helmand lake region around Zabol at the Afghan-Iranian border.</obo:IAO_0000115>
        <oboInOwl:hasOBONamespace>GAZ</oboInOwl:hasOBONamespace>
        <oboInOwl:id>GAZ:00148844</oboInOwl:id>
        <rdfs:label>Helmand River</rdfs:label>
    </owl:NamedIndividual>
    


    <!-- http://purl.obolibrary.org/obo/GAZ_00148845 -->

    <owl:NamedIndividual rdf:about="http://purl.obolibrary.org/obo/GAZ_00148845">
        <obo:RO_0001025 rdf:resource="http://purl.obolibrary.org/obo/GAZ_00148844"/>
        <obo:IAO_0000115>A dam and associated reservoir located 55 miles north-west of Kandahar City.</obo:IAO_0000115>
        <oboInOwl:hasOBONamespace>GAZ</oboInOwl:hasOBONamespace>
        <oboInOwl:id>GAZ:00148845</oboInOwl:id>
        <rdfs:label>Kajaki Dam</rdfs:label>
    </owl:NamedIndividual>
    


    <!-- http://purl.obolibrary.org/obo/GAZ_00148846 -->

    <owl:NamedIndividual rdf:about="http://purl.obolibrary.org/obo/GAZ_00148846">
        <obo:RO_0001025 rdf:resource="http://purl.obolibrary.org/obo/GAZ_00148844"/>
        <obo:IAO_0000115>A dam on the Helmand River in Helmand Province of Afghanistan.</obo:IAO_0000115>
        <oboInOwl:hasOBONamespace>GAZ</oboInOwl:hasOBONamespace>
        <oboInOwl:id>GAZ:00148846</oboInOwl:id>
        <rdfs:label>Grishk Dam</rdfs:label>
    </owl:NamedIndividual>
    


    <!-- http://purl.obolibrary.org/obo/GAZ_00148865 -->

    <owl:NamedIndividual rdf:about="http://purl.obolibrary.org/obo/GAZ_00148865">
        <obo:IAO_0000115>A dam on the Chambal in Neemuch District of Madhya Pradesh.</obo:IAO_0000115>
        <oboInOwl:hasOBONamespace>GAZ</oboInOwl:hasOBONamespace>
        <oboInOwl:id>GAZ:00148865</oboInOwl:id>
        <rdfs:label>Gandhi Sagar Dam</rdfs:label>
    </owl:NamedIndividual>
    


    <!-- http://purl.obolibrary.org/obo/GAZ_00148866 -->

    <owl:NamedIndividual rdf:about="http://purl.obolibrary.org/obo/GAZ_00148866">
        <obo:IAO_0000115>A dam located 52 km downstream of Gandhi Sagar dam on across the Chambal River near Rawatbhata in Chittorgarh district in Rajasthan. Completed 1970.</obo:IAO_0000115>
        <oboInOwl:hasOBONamespace>GAZ</oboInOwl:hasOBONamespace>
        <oboInOwl:id>GAZ:00148866</oboInOwl:id>
        <rdfs:label>Rana Pratap Sagar Dam</rdfs:label>
    </owl:NamedIndividual>
    


    <!-- http://purl.obolibrary.org/obo/GAZ_00148867 -->

    <owl:NamedIndividual rdf:about="http://purl.obolibrary.org/obo/GAZ_00148867">
        <obo:IAO_0000115>A dam located about 0.8 km upstream of Kota City in Rajasthan.</obo:IAO_0000115>
        <oboInOwl:hasOBONamespace>GAZ</oboInOwl:hasOBONamespace>
        <oboInOwl:id>GAZ:00148867</oboInOwl:id>
        <rdfs:label>Kota Barrage</rdfs:label>
    </owl:NamedIndividual>
    


    <!-- http://purl.obolibrary.org/obo/GAZ_00148868 -->

    <owl:NamedIndividual rdf:about="http://purl.obolibrary.org/obo/GAZ_00148868">
        <obo:IAO_0000115>A dam across the Chambal River. It is situated 24 km south-west of Kota, Rajasthan.</obo:IAO_0000115>
        <oboInOwl:hasOBONamespace>GAZ</oboInOwl:hasOBONamespace>
        <oboInOwl:id>GAZ:00148868</oboInOwl:id>
        <rdfs:label>Jawahar Sagar Dam</rdfs:label>
    </owl:NamedIndividual>
    


    <!-- http://purl.obolibrary.org/obo/GAZ_00148909 -->

    <owl:NamedIndividual rdf:about="http://purl.obolibrary.org/obo/GAZ_00148909">
        <obo:IAO_0000115>An Inter-state Dam project of the Government of Madhya Pradesh and Uttar Pradesh being constructed on Betwa River about 22 km from Lalitpur in Uttar Pradesh, India.</obo:IAO_0000115>
        <oboInOwl:hasOBONamespace>GAZ</oboInOwl:hasOBONamespace>
        <oboInOwl:id>GAZ:00148909</oboInOwl:id>
        <rdfs:label>Rajghat Dam</rdfs:label>
    </owl:NamedIndividual>
    


    <!-- http://purl.obolibrary.org/obo/GAZ_00148911 -->

    <owl:NamedIndividual rdf:about="http://purl.obolibrary.org/obo/GAZ_00148911">
        <obo:IAO_0000115>A reservoir being created by the Rajghat Dam.</obo:IAO_0000115>
        <oboInOwl:hasOBONamespace>GAZ</oboInOwl:hasOBONamespace>
        <oboInOwl:id>GAZ:00148911</oboInOwl:id>
        <rdfs:label>Rajghat Reservoir</rdfs:label>
    </owl:NamedIndividual>
    


    <!-- http://purl.obolibrary.org/obo/GAZ_00148912 -->

    <owl:NamedIndividual rdf:about="http://purl.obolibrary.org/obo/GAZ_00148912">
        <obo:IAO_0000115>A dam in India on the Betwa River. Situated 93 km away from Deogarh, Uttar Pradesh. Constructed 1958.</obo:IAO_0000115>
        <oboInOwl:hasOBONamespace>GAZ</oboInOwl:hasOBONamespace>
        <oboInOwl:id>GAZ:00148912</oboInOwl:id>
        <rdfs:label>Matatila Dam</rdfs:label>
    </owl:NamedIndividual>
    


    <!-- http://purl.obolibrary.org/obo/GAZ_00148913 -->

    <owl:NamedIndividual rdf:about="http://purl.obolibrary.org/obo/GAZ_00148913">
        <obo:IAO_0000115>A dam built on the Betwa River near Parichha town, Uttar Pradesh.</obo:IAO_0000115>
        <oboInOwl:hasOBONamespace>GAZ</oboInOwl:hasOBONamespace>
        <oboInOwl:id>GAZ:00148913</oboInOwl:id>
        <rdfs:label>Parichha Dam</rdfs:label>
    </owl:NamedIndividual>
    


    <!-- http://purl.obolibrary.org/obo/GAZ_00148924 -->

    <owl:NamedIndividual rdf:about="http://purl.obolibrary.org/obo/GAZ_00148924">
        <obo:IAO_0000115>A multi-purpose dam situated in Shivpuri district in Madhya Pradesh, India. Impounds the Madikheda Reservoir. Constructed 1978-2008.</obo:IAO_0000115>
        <oboInOwl:hasOBONamespace>GAZ</oboInOwl:hasOBONamespace>
        <oboInOwl:id>GAZ:00148924</oboInOwl:id>
        <rdfs:label>Madikheda Dam</rdfs:label>
    </owl:NamedIndividual>
    


    <!-- http://purl.obolibrary.org/obo/GAZ_00148925 -->

    <owl:NamedIndividual rdf:about="http://purl.obolibrary.org/obo/GAZ_00148925">
        <obo:IAO_0000115>A reservoir created by the Madikheda Dam. Constructed 1978-2008.</obo:IAO_0000115>
        <oboInOwl:hasOBONamespace>GAZ</oboInOwl:hasOBONamespace>
        <oboInOwl:id>GAZ:00148925</oboInOwl:id>
        <rdfs:label>Madikheda Reservoir</rdfs:label>
    </owl:NamedIndividual>
    


    <!-- http://purl.obolibrary.org/obo/GAZ_00149036 -->

    <owl:NamedIndividual rdf:about="http://purl.obolibrary.org/obo/GAZ_00149036">
        <obo:IAO_0000115>A dam located in Yamuna Nagar District, in the State of Haryana, India. It regulates the flow of the Yamuna for irrigation in Uttar Pradesh and Haryana through two canals originating at this place namely Western Yamuna Canal and Eastern Yamuna Canal, as well as the municipal water supply to Delhi. Completed 1873.</obo:IAO_0000115>
        <oboInOwl:hasOBONamespace>GAZ</oboInOwl:hasOBONamespace>
        <oboInOwl:id>GAZ:00149036</oboInOwl:id>
        <rdfs:label>Tajewala Dam</rdfs:label>
    </owl:NamedIndividual>
    


    <!-- http://purl.obolibrary.org/obo/GAZ_00149059 -->

    <owl:NamedIndividual rdf:about="http://purl.obolibrary.org/obo/GAZ_00149059">
        <obo:RO_0001025 rdf:resource="http://purl.obolibrary.org/obo/GAZ_00149060"/>
        <obo:IAO_0000115>A glacier situated in the Pithoragarh District of Uttarakhand State of India The glacier situated on Kumaon Himalayas at an altitude of 3,600 m.</obo:IAO_0000115>
        <oboInOwl:hasOBONamespace>GAZ</oboInOwl:hasOBONamespace>
        <oboInOwl:id>GAZ:00149059</oboInOwl:id>
        <rdfs:label>Namik Glacier</rdfs:label>
    </owl:NamedIndividual>
    


    <!-- http://purl.obolibrary.org/obo/GAZ_00149060 -->

    <owl:NamedIndividual rdf:about="http://purl.obolibrary.org/obo/GAZ_00149060">
        <oboInOwl:hasOBONamespace>GAZ</oboInOwl:hasOBONamespace>
        <oboInOwl:id>GAZ:00149060</oboInOwl:id>
        <rdfs:label>Kumaon Himalayas</rdfs:label>
    </owl:NamedIndividual>
    


    <!-- http://purl.obolibrary.org/obo/GAZ_00149073 -->

    <owl:NamedIndividual rdf:about="http://purl.obolibrary.org/obo/GAZ_00149073">
        <obo:IAO_0000115>A below water construction on Betwa River near Jhansi District, Uttar Pradesh.</obo:IAO_0000115>
        <oboInOwl:hasOBONamespace>GAZ</oboInOwl:hasOBONamespace>
        <oboInOwl:id>GAZ:00149073</oboInOwl:id>
        <rdfs:label>Sukma-Dukma Dam</rdfs:label>
    </owl:NamedIndividual>
    


    <!-- http://purl.obolibrary.org/obo/GAZ_00149194 -->

    <owl:NamedIndividual rdf:about="http://purl.obolibrary.org/obo/GAZ_00149194">
        <obo:RO_0001025 rdf:resource="http://purl.obolibrary.org/obo/GAZ_00005246"/>
        <obo:IAO_0000115>A river in Pakistan originating in India. It originates in the Himalayas in the Chamba district of Himachal Pradesh following a north-westerly course. It turns to the south-west, near Dalhousie, and then cuts a gorge in the Dhaola Dhar range entering the Punjab plain near Madhopur near pathankot. It then flows along the Indo-Pakistan border for some distance before entering Pakistan and joining the Chenab River.</obo:IAO_0000115>
        <oboInOwl:hasOBONamespace>GAZ</oboInOwl:hasOBONamespace>
        <oboInOwl:id>GAZ:00149194</oboInOwl:id>
        <rdfs:label>Ravi River</rdfs:label>
    </owl:NamedIndividual>
    


    <!-- http://purl.obolibrary.org/obo/GAZ_00149195 -->

    <owl:NamedIndividual rdf:about="http://purl.obolibrary.org/obo/GAZ_00149195">
        <obo:RO_0001025 rdf:resource="http://purl.obolibrary.org/obo/GAZ_00149194"/>
        <obo:IAO_0000115>A dam on the Ravi River, near Chamba, Himachal Pradesh.</obo:IAO_0000115>
        <oboInOwl:hasOBONamespace>GAZ</oboInOwl:hasOBONamespace>
        <oboInOwl:id>GAZ:00149195</oboInOwl:id>
        <rdfs:label>Chamera Dam</rdfs:label>
    </owl:NamedIndividual>
    


    <!-- http://purl.obolibrary.org/obo/GAZ_00149226 -->

    <owl:NamedIndividual rdf:about="http://purl.obolibrary.org/obo/GAZ_00149226">
        <obo:RO_0001025 rdf:resource="http://purl.obolibrary.org/obo/GAZ_00248810"/>
        <obo:IAO_0000115>A protected area located in eastern Haryana, India, 150 km from Chandigarh.</obo:IAO_0000115>
        <oboInOwl:hasOBONamespace>GAZ</oboInOwl:hasOBONamespace>
        <oboInOwl:id>GAZ:00149226</oboInOwl:id>
        <rdfs:label>Kalesar National Park</rdfs:label>
    </owl:NamedIndividual>
    


    <!-- http://purl.obolibrary.org/obo/GAZ_00149534 -->

    <owl:NamedIndividual rdf:about="http://purl.obolibrary.org/obo/GAZ_00149534">
        <obo:IAO_0000115>A high altitude wildlife sanctuary located in the easternmost reaches of the Karakoram range in Leh District, Jammu and Kashmir.</obo:IAO_0000115>
        <oboInOwl:hasOBONamespace>GAZ</oboInOwl:hasOBONamespace>
        <oboInOwl:id>GAZ:00149534</oboInOwl:id>
        <rdfs:label>Karakoram Wildlife Sanctuary</rdfs:label>
    </owl:NamedIndividual>
    


    <!-- http://purl.obolibrary.org/obo/GAZ_00149894 -->

    <owl:NamedIndividual rdf:about="http://purl.obolibrary.org/obo/GAZ_00149894">
        <obo:RO_0001025 rdf:resource="http://purl.obolibrary.org/obo/GAZ_00056948"/>
        <obo:IAO_0000115>A protected area situated in the west Indian State of Rajasthan near the town of Jaisalmer.</obo:IAO_0000115>
        <oboInOwl:hasOBONamespace>GAZ</oboInOwl:hasOBONamespace>
        <oboInOwl:id>GAZ:00149894</oboInOwl:id>
        <rdfs:label>Desert National Park</rdfs:label>
    </owl:NamedIndividual>
    


    <!-- http://purl.obolibrary.org/obo/GAZ_00150304 -->

    <owl:NamedIndividual rdf:about="http://purl.obolibrary.org/obo/GAZ_00150304">
        <obo:IAO_0000115>A glacier located in the eastern Karakoram range in the Himalaya Mountains. The glacier&apos;s melting waters are the main source of the Nubra River, which drains into the Shyok River. The Shyok in turn joins the Indus River, thus the glacier is a major source of the river Indus.</obo:IAO_0000115>
        <oboInOwl:hasOBONamespace>GAZ</oboInOwl:hasOBONamespace>
        <oboInOwl:id>GAZ:00150304</oboInOwl:id>
        <rdfs:label>Siachen Glacier</rdfs:label>
    </owl:NamedIndividual>
    


    <!-- http://purl.obolibrary.org/obo/GAZ_00246580 -->

    <owl:NamedIndividual rdf:about="http://purl.obolibrary.org/obo/GAZ_00246580">
        <obo:RO_0001025 rdf:resource="http://purl.obolibrary.org/obo/GAZ_00004988"/>
        <obo:IAO_0000115>A high altitude lake. Located some 45 km southeast of Zorkul. It lies in a broad valley between the Big Pamir and Small Pamir ranges, and is fed by snow-melt from both these ranges. It is about 16 km long and up to 2 km wide. The lake drains through an outlet at its eastern end into the Aksu River, which joins the Pamir River in Tadzhikistan.</obo:IAO_0000115>
        <oboInOwl:hasOBONamespace>GAZ</oboInOwl:hasOBONamespace>
        <oboInOwl:id>GAZ:00246580</oboInOwl:id>
        <rdfs:label>Chaqmatin Lake</rdfs:label>
    </owl:NamedIndividual>
    


    <!-- http://purl.obolibrary.org/obo/GAZ_00246584 -->

    <owl:NamedIndividual rdf:about="http://purl.obolibrary.org/obo/GAZ_00246584">
        <obo:IAO_0000115>A lake created by a barrage on the Kabul River.</obo:IAO_0000115>
        <oboInOwl:hasOBONamespace>GAZ</oboInOwl:hasOBONamespace>
        <oboInOwl:id>GAZ:00246584</oboInOwl:id>
        <rdfs:label>Lake Sarobi</rdfs:label>
    </owl:NamedIndividual>
    


    <!-- http://purl.obolibrary.org/obo/GAZ_00246586 -->

    <owl:NamedIndividual rdf:about="http://purl.obolibrary.org/obo/GAZ_00246586">
        <obo:RO_0001025 rdf:resource="http://purl.obolibrary.org/obo/GAZ_00246588"/>
        <obo:IAO_0000115>A high desert plateau, about 40 km from north to south and up to 15 km from east to west, in the Koh-i Baba Range of the Hindu Kush. It is surrounded on all sides by mountains rising to peaks in excess of 4,800 m, and contains a shallow, brackish lake, Ab-i Nawar.</obo:IAO_0000115>
        <oboInOwl:hasOBONamespace>GAZ</oboInOwl:hasOBONamespace>
        <oboInOwl:id>GAZ:00246586</oboInOwl:id>
        <rdfs:label>Dashte Nawar</rdfs:label>
    </owl:NamedIndividual>
    


    <!-- http://purl.obolibrary.org/obo/GAZ_00246587 -->

    <owl:NamedIndividual rdf:about="http://purl.obolibrary.org/obo/GAZ_00246587">
        <obo:RO_0001025 rdf:resource="http://purl.obolibrary.org/obo/GAZ_00246586"/>
        <obo:IAO_0000115>A shallow brackish lake.</obo:IAO_0000115>
        <oboInOwl:hasOBONamespace>GAZ</oboInOwl:hasOBONamespace>
        <oboInOwl:id>GAZ:00246587</oboInOwl:id>
        <rdfs:label>Ab-i Nawar</rdfs:label>
    </owl:NamedIndividual>
    


    <!-- http://purl.obolibrary.org/obo/GAZ_00246588 -->

    <owl:NamedIndividual rdf:about="http://purl.obolibrary.org/obo/GAZ_00246588">
        <obo:RO_0001025 rdf:resource="http://purl.obolibrary.org/obo/GAZ_00056902"/>
        <obo:IAO_0000115>A mountain range.</obo:IAO_0000115>
        <oboInOwl:hasOBONamespace>GAZ</oboInOwl:hasOBONamespace>
        <oboInOwl:id>GAZ:00246588</oboInOwl:id>
        <rdfs:label>Koh-i Baba Range</rdfs:label>
    </owl:NamedIndividual>
    


    <!-- http://purl.obolibrary.org/obo/GAZ_00246589 -->

    <owl:NamedIndividual rdf:about="http://purl.obolibrary.org/obo/GAZ_00246589">
        <obo:IAO_0000115>A large alkaline lake in the southern foothills of the Hindu Kush. It lies on a gently rolling plateau in the southern foothills of the Koh-i Baba and Koh-i Paghman ranges.</obo:IAO_0000115>
        <oboInOwl:hasOBONamespace>GAZ</oboInOwl:hasOBONamespace>
        <oboInOwl:id>GAZ:00246589</oboInOwl:id>
        <rdfs:label>Ab-i Istada</rdfs:label>
    </owl:NamedIndividual>
    


    <!-- http://purl.obolibrary.org/obo/GAZ_00246590 -->

    <owl:NamedIndividual rdf:about="http://purl.obolibrary.org/obo/GAZ_00246590">
        <obo:RO_0001025 rdf:resource="http://purl.obolibrary.org/obo/GAZ_00056902"/>
        <obo:IAO_0000115>A mountain range.</obo:IAO_0000115>
        <oboInOwl:hasOBONamespace>GAZ</oboInOwl:hasOBONamespace>
        <oboInOwl:id>GAZ:00246590</oboInOwl:id>
        <rdfs:label>Koh-i Paghman Range</rdfs:label>
    </owl:NamedIndividual>
    


    <!-- http://purl.obolibrary.org/obo/GAZ_00247596 -->

    <owl:NamedIndividual rdf:about="http://purl.obolibrary.org/obo/GAZ_00247596">
        <obo:IAO_0000115>A large, deep, freshwater lake and associated marshes in the mountains southwest of Lasa.</obo:IAO_0000115>
        <oboInOwl:hasOBONamespace>GAZ</oboInOwl:hasOBONamespace>
        <oboInOwl:id>GAZ:00247596</oboInOwl:id>
        <rdfs:label>Yangcaoyong Cuo</rdfs:label>
    </owl:NamedIndividual>
    


    <!-- http://purl.obolibrary.org/obo/GAZ_00247597 -->

    <owl:NamedIndividual rdf:about="http://purl.obolibrary.org/obo/GAZ_00247597">
        <obo:IAO_0000115>A large freshwater lake and associated marshes on the north slope of the main Himalayan range. Located 135 km southwest of Lasa, Xizang Zizhiqu.</obo:IAO_0000115>
        <oboInOwl:hasOBONamespace>GAZ</oboInOwl:hasOBONamespace>
        <oboInOwl:id>GAZ:00247597</oboInOwl:id>
        <rdfs:label>Pumuoyong Cuo</rdfs:label>
    </owl:NamedIndividual>
    


    <!-- http://purl.obolibrary.org/obo/GAZ_00247598 -->

    <owl:NamedIndividual rdf:about="http://purl.obolibrary.org/obo/GAZ_00247598">
        <obo:IAO_0000115>A large, brackish or saline lake in an inland drainage basin on the north slope of the main Himalayan range. The lake is fed by snowmelt from the Xixabangma Feng Mountains to the south (peaks to 8,012m). Located south of the Yarlung Zangbo Jiang (Brahmaputra River), 540 km west of Lasa.</obo:IAO_0000115>
        <oboInOwl:hasOBONamespace>GAZ</oboInOwl:hasOBONamespace>
        <oboInOwl:id>GAZ:00247598</oboInOwl:id>
        <rdfs:label>Paiku Co</rdfs:label>
    </owl:NamedIndividual>
    


    <!-- http://purl.obolibrary.org/obo/GAZ_00247601 -->

    <owl:NamedIndividual rdf:about="http://purl.obolibrary.org/obo/GAZ_00247601">
        <obo:IAO_0000115>A chain of four interconnected lakes. Located at the east end of the Karakoram Range, on the border between China and India, Xizang Zizhiqu (Tibetan Autonomous Region) and Jammu &amp; Kashmir (India).</obo:IAO_0000115>
        <oboInOwl:hasOBONamespace>GAZ</oboInOwl:hasOBONamespace>
        <oboInOwl:id>GAZ:00247601</oboInOwl:id>
        <rdfs:label>Pangong Lakes</rdfs:label>
    </owl:NamedIndividual>
    


    <!-- http://purl.obolibrary.org/obo/GAZ_00248628 -->

    <owl:NamedIndividual rdf:about="http://purl.obolibrary.org/obo/GAZ_00248628">
        <obo:IAO_0000115>A major which flows through the north-western part of South Asia. Originating in the Tibetan plateau in the vicinity of Lake Mansarovar in Tibet Autonomous Region, the river runs a course through the Ladakh district of Jammu and Kashmir and then enters Northern Areas (Gilgit-Baltistan), flowing through the North in a southerly direction along the entire length of the country, to merge into the Arabian Sea near port city of Karachi in Sindh. Together with the rivers Chenab, Ravi, Sutlej, Jhelum, Beas and two tributaries from the North West Frontier and Afghanistan, the Indus forms the Sapta Sindhu (Seven Rivers) delta of Pakistan.</obo:IAO_0000115>
        <oboInOwl:hasOBONamespace>GAZ</oboInOwl:hasOBONamespace>
        <oboInOwl:id>GAZ:00248628</oboInOwl:id>
        <rdfs:label>Indus River</rdfs:label>
    </owl:NamedIndividual>
    


    <!-- http://purl.obolibrary.org/obo/GAZ_00248630 -->

    <owl:NamedIndividual rdf:about="http://purl.obolibrary.org/obo/GAZ_00248630">
        <obo:IAO_0000115>A river. A tributary of the Shyok River, which flows into the Indus River. It flows in the Ladakh area of Jammu and Kashmir.</obo:IAO_0000115>
        <oboInOwl:hasOBONamespace>GAZ</oboInOwl:hasOBONamespace>
        <oboInOwl:id>GAZ:00248630</oboInOwl:id>
        <rdfs:label>Nubra River</rdfs:label>
    </owl:NamedIndividual>
    


    <!-- http://purl.obolibrary.org/obo/GAZ_00248632 -->

    <owl:NamedIndividual rdf:about="http://purl.obolibrary.org/obo/GAZ_00248632">
        <obo:RO_0001025 rdf:resource="http://purl.obolibrary.org/obo/GAZ_00018580"/>
        <obo:IAO_0000115>A valley in Baltistan in northern Pakistan that is watered by Shigar River. The valley stretches about 170km from Skardu to Askole and is the gateway to the high mountains of the Karakoram. Shigar is the administrative sub-division of District Skardu.</obo:IAO_0000115>
        <oboInOwl:hasOBONamespace>GAZ</oboInOwl:hasOBONamespace>
        <oboInOwl:id>GAZ:00248632</oboInOwl:id>
        <rdfs:label>Shigar Valley</rdfs:label>
    </owl:NamedIndividual>
    


    <!-- http://purl.obolibrary.org/obo/GAZ_00248636 -->

    <owl:NamedIndividual rdf:about="http://purl.obolibrary.org/obo/GAZ_00248636">
        <obo:RO_0001025 rdf:resource="http://purl.obolibrary.org/obo/GAZ_00005256"/>
        <obo:IAO_0000115>A lake. The source of the Giglit River.</obo:IAO_0000115>
        <oboInOwl:hasOBONamespace>GAZ</oboInOwl:hasOBONamespace>
        <oboInOwl:id>GAZ:00248636</oboInOwl:id>
        <rdfs:label>Lake Shandur</rdfs:label>
    </owl:NamedIndividual>
    


    <!-- http://purl.obolibrary.org/obo/GAZ_00248645 -->

    <owl:NamedIndividual rdf:about="http://purl.obolibrary.org/obo/GAZ_00248645">
        <obo:RO_0001025 rdf:resource="http://purl.obolibrary.org/obo/GAZ_00005249"/>
        <obo:IAO_0000115>A river in Punjab, Pakistan. Panjnad River is formed by successive confluence of the five rivers of Punjab, namely Jhelum, Chenab, Ravi, Beas and Sutlej. Jhelum and Ravi join Chenab, Beas joins Sutlej, and then Sutlej and Chenab join to form Panjnad 10 miles north of Uch Sharif. The combined stream runs southwest for approximately 45 miles and joins Indus River at Mithankot.</obo:IAO_0000115>
        <oboInOwl:hasOBONamespace>GAZ</oboInOwl:hasOBONamespace>
        <oboInOwl:id>GAZ:00248645</oboInOwl:id>
        <rdfs:label>Panjnad River</rdfs:label>
    </owl:NamedIndividual>
    


    <!-- http://purl.obolibrary.org/obo/GAZ_00248646 -->

    <owl:NamedIndividual rdf:about="http://purl.obolibrary.org/obo/GAZ_00248646">
        <obo:RO_0001025 rdf:resource="http://purl.obolibrary.org/obo/GAZ_00080566"/>
        <obo:IAO_0000115>A populated place. A located in southern Punjab, Pakistan.</obo:IAO_0000115>
        <oboInOwl:hasOBONamespace>GAZ</oboInOwl:hasOBONamespace>
        <oboInOwl:id>GAZ:00248646</oboInOwl:id>
        <rdfs:label>Mithankot</rdfs:label>
    </owl:NamedIndividual>
    


    <!-- http://purl.obolibrary.org/obo/GAZ_00248649 -->

    <owl:NamedIndividual rdf:about="http://purl.obolibrary.org/obo/GAZ_00248649">
        <obo:RO_0001025 rdf:resource="http://purl.obolibrary.org/obo/GAZ_00148807"/>
        <obo:IAO_0000115>A concrete gravity dam across the Sutlej River, near the border between Punjab and Himachal Pradesh in northern India. Completed 1963.</obo:IAO_0000115>
        <oboInOwl:hasOBONamespace>GAZ</oboInOwl:hasOBONamespace>
        <oboInOwl:id>GAZ:00248649</oboInOwl:id>
        <rdfs:label>Bhakra Nangal Dam</rdfs:label>
    </owl:NamedIndividual>
    


    <!-- http://purl.obolibrary.org/obo/GAZ_00248650 -->

    <owl:NamedIndividual rdf:about="http://purl.obolibrary.org/obo/GAZ_00248650">
        <rdf:type rdf:resource="http://purl.obolibrary.org/obo/ENVO_00000856"/>
        <obo:RO_0001025 rdf:resource="http://purl.obolibrary.org/obo/GAZ_00400079"/>
        <obo:IAO_0000115>A populated place. A small town at the intersection of the rivers Jhelum and Chenab in Jhang District, Punjab, Pakistan.</obo:IAO_0000115>
        <oboInOwl:hasOBONamespace>GAZ</oboInOwl:hasOBONamespace>
        <oboInOwl:id>GAZ:00248650</oboInOwl:id>
        <rdfs:label>Atharan Hazari</rdfs:label>
    </owl:NamedIndividual>
    


    <!-- http://purl.obolibrary.org/obo/GAZ_00248652 -->

    <owl:NamedIndividual rdf:about="http://purl.obolibrary.org/obo/GAZ_00248652">
        <obo:RO_0001025 rdf:resource="http://purl.obolibrary.org/obo/GAZ_00080602"/>
        <obo:IAO_0000115>A populated place. The capital of Azad Kashmir. It is located in Muzaffarabad District on the banks of the Jhelum and Neelum rivers.</obo:IAO_0000115>
        <oboInOwl:hasOBONamespace>GAZ</oboInOwl:hasOBONamespace>
        <oboInOwl:id>GAZ:00248652</oboInOwl:id>
        <rdfs:label>Muzaffarabad</rdfs:label>
    </owl:NamedIndividual>
    


    <!-- http://purl.obolibrary.org/obo/GAZ_00248653 -->

    <owl:NamedIndividual rdf:about="http://purl.obolibrary.org/obo/GAZ_00248653">
        <obo:IAO_0000115>A river located in North-West Frontier Province, Pakistan. The river originates from Lulusar lake, nearly 48km from Naran Valley. Waters of Dudipat and Saiful Muluk lakes feed the river besides glacial waters from Malka Parbat and other high peaks in the valley. Kunhar flows through entire Kaghan Valley through Jalkhad, Naran, Kaghan, Balakot, Garhi Habibullah and joins Jhelum River just outside Muzaffarabad in Azad Jammu and Kashmir.</obo:IAO_0000115>
        <oboInOwl:hasOBONamespace>GAZ</oboInOwl:hasOBONamespace>
        <oboInOwl:id>GAZ:00248653</oboInOwl:id>
        <rdfs:label>Kunhar River</rdfs:label>
    </owl:NamedIndividual>
    


    <!-- http://purl.obolibrary.org/obo/GAZ_00248654 -->

    <owl:NamedIndividual rdf:about="http://purl.obolibrary.org/obo/GAZ_00248654">
        <rdf:type rdf:resource="http://purl.obolibrary.org/obo/ENVO_00000856"/>
        <obo:RO_0001025 rdf:resource="http://purl.obolibrary.org/obo/GAZ_00058423"/>
        <obo:IAO_0000115>A populated place. A village located in Kaghan Valley of Mansehra District, North-West Frontier Province, Pakistan.</obo:IAO_0000115>
        <oboInOwl:hasOBONamespace>GAZ</oboInOwl:hasOBONamespace>
        <oboInOwl:id>GAZ:00248654</oboInOwl:id>
        <rdfs:label>Naran Village</rdfs:label>
    </owl:NamedIndividual>
    


    <!-- http://purl.obolibrary.org/obo/GAZ_00248655 -->

    <owl:NamedIndividual rdf:about="http://purl.obolibrary.org/obo/GAZ_00248655">
        <rdf:type rdf:resource="http://purl.obolibrary.org/obo/ENVO_00000856"/>
        <obo:RO_0001025 rdf:resource="http://purl.obolibrary.org/obo/GAZ_00058423"/>
        <obo:RO_0001025 rdf:resource="http://purl.obolibrary.org/obo/GAZ_00248656"/>
        <obo:IAO_0000115>A populated place. A small town of the Balakot Tehsil, in Mansehra District of North-West Frontier Province, Pakistan.</obo:IAO_0000115>
        <oboInOwl:hasOBONamespace>GAZ</oboInOwl:hasOBONamespace>
        <oboInOwl:id>GAZ:00248655</oboInOwl:id>
        <rdfs:label>Kaghan</rdfs:label>
    </owl:NamedIndividual>
    


    <!-- http://purl.obolibrary.org/obo/GAZ_00248656 -->

    <owl:NamedIndividual rdf:about="http://purl.obolibrary.org/obo/GAZ_00248656">
        <obo:RO_0001025 rdf:resource="http://purl.obolibrary.org/obo/GAZ_00080442"/>
        <obo:IAO_0000115>A union council of the Balakot Tehsil, in Mansehra District of North-West Frontier Province, Pakistan.</obo:IAO_0000115>
        <oboInOwl:hasOBONamespace>GAZ</oboInOwl:hasOBONamespace>
        <oboInOwl:id>GAZ:00248656</oboInOwl:id>
        <rdfs:label>Kaghan Union Council</rdfs:label>
    </owl:NamedIndividual>
    


    <!-- http://purl.obolibrary.org/obo/GAZ_00248657 -->

    <owl:NamedIndividual rdf:about="http://purl.obolibrary.org/obo/GAZ_00248657">
        <obo:RO_0001025 rdf:resource="http://purl.obolibrary.org/obo/GAZ_00080442"/>
        <obo:IAO_0000115>A Union Council.</obo:IAO_0000115>
        <oboInOwl:hasOBONamespace>GAZ</oboInOwl:hasOBONamespace>
        <oboInOwl:id>GAZ:00248657</oboInOwl:id>
        <rdfs:label>Balakot Union Council</rdfs:label>
    </owl:NamedIndividual>
    


    <!-- http://purl.obolibrary.org/obo/GAZ_00248658 -->

    <owl:NamedIndividual rdf:about="http://purl.obolibrary.org/obo/GAZ_00248658">
        <rdf:type rdf:resource="http://purl.obolibrary.org/obo/ENVO_00000856"/>
        <obo:RO_0001025 rdf:resource="http://purl.obolibrary.org/obo/GAZ_00248657"/>
        <obo:IAO_0000115>A populated place. A town in Mansehra District in the North-West Frontier Province of Pakistan.</obo:IAO_0000115>
        <oboInOwl:hasOBONamespace>GAZ</oboInOwl:hasOBONamespace>
        <oboInOwl:id>GAZ:00248658</oboInOwl:id>
        <rdfs:label>Balakot</rdfs:label>
    </owl:NamedIndividual>
    


    <!-- http://purl.obolibrary.org/obo/GAZ_00248659 -->

    <owl:NamedIndividual rdf:about="http://purl.obolibrary.org/obo/GAZ_00248659">
        <obo:RO_0001025 rdf:resource="http://purl.obolibrary.org/obo/GAZ_00080445"/>
        <obo:IAO_0000115>A Union Council.</obo:IAO_0000115>
        <oboInOwl:hasOBONamespace>GAZ</oboInOwl:hasOBONamespace>
        <oboInOwl:id>GAZ:00248659</oboInOwl:id>
        <rdfs:label>Garhi Habibullah Union Council</rdfs:label>
    </owl:NamedIndividual>
    


    <!-- http://purl.obolibrary.org/obo/GAZ_00248660 -->

    <owl:NamedIndividual rdf:about="http://purl.obolibrary.org/obo/GAZ_00248660">
        <rdf:type rdf:resource="http://purl.obolibrary.org/obo/ENVO_00000856"/>
        <obo:RO_0001025 rdf:resource="http://purl.obolibrary.org/obo/GAZ_00248659"/>
        <obo:IAO_0000115>A populated place. A town off Mansehra District in the North-West Frontier Province of Pakistan.</obo:IAO_0000115>
        <oboInOwl:hasOBONamespace>GAZ</oboInOwl:hasOBONamespace>
        <oboInOwl:id>GAZ:00248660</oboInOwl:id>
        <rdfs:label>Garhi Habibullah</rdfs:label>
    </owl:NamedIndividual>
    


    <!-- http://purl.obolibrary.org/obo/GAZ_00248662 -->

    <owl:NamedIndividual rdf:about="http://purl.obolibrary.org/obo/GAZ_00248662">
        <obo:RO_0001025 rdf:resource="http://purl.obolibrary.org/obo/GAZ_00018568"/>
        <obo:IAO_0000115>A dam located in Mirpur District. Constructed 1967.</obo:IAO_0000115>
        <oboInOwl:hasOBONamespace>GAZ</oboInOwl:hasOBONamespace>
        <oboInOwl:id>GAZ:00248662</oboInOwl:id>
        <rdfs:label>Mangla Dam</rdfs:label>
    </owl:NamedIndividual>
    


    <!-- http://purl.obolibrary.org/obo/GAZ_00248663 -->

    <owl:NamedIndividual rdf:about="http://purl.obolibrary.org/obo/GAZ_00248663">
        <obo:RO_0001025 rdf:resource="http://purl.obolibrary.org/obo/GAZ_00248650"/>
        <obo:IAO_0000115>A flood control mechanism which was constructed to protect the city of Jhang from floods. At the confluence of the Chenab and Jhelum Rivers.</obo:IAO_0000115>
        <oboInOwl:hasOBONamespace>GAZ</oboInOwl:hasOBONamespace>
        <oboInOwl:id>GAZ:00248663</oboInOwl:id>
        <rdfs:label>Head Trimmu</rdfs:label>
    </owl:NamedIndividual>
    


    <!-- http://purl.obolibrary.org/obo/GAZ_00248664 -->

    <owl:NamedIndividual rdf:about="http://purl.obolibrary.org/obo/GAZ_00248664">
        <obo:RO_0001025 rdf:resource="http://purl.obolibrary.org/obo/GAZ_00400071"/>
        <obo:IAO_0000115>A flood control mechanism.</obo:IAO_0000115>
        <oboInOwl:hasOBONamespace>GAZ</oboInOwl:hasOBONamespace>
        <oboInOwl:id>GAZ:00248664</oboInOwl:id>
        <rdfs:label>Head Khanki</rdfs:label>
    </owl:NamedIndividual>
    


    <!-- http://purl.obolibrary.org/obo/GAZ_00248665 -->

    <owl:NamedIndividual rdf:about="http://purl.obolibrary.org/obo/GAZ_00248665">
        <obo:RO_0001025 rdf:resource="http://purl.obolibrary.org/obo/GAZ_00400071"/>
        <obo:IAO_0000115>A canal in Pakistan. It originates from Head Khanki, which is situated at the Chenab river in the Gujrat district. Some distributaries coming out of Lower Chenab are the Jhang Branch, the Rakh Branch and the Gugera Branch Canal. Constructed 1892.</obo:IAO_0000115>
        <oboInOwl:hasOBONamespace>GAZ</oboInOwl:hasOBONamespace>
        <oboInOwl:id>GAZ:00248665</oboInOwl:id>
        <rdfs:label>Lower Chenab Canal</rdfs:label>
    </owl:NamedIndividual>
    


    <!-- http://purl.obolibrary.org/obo/GAZ_00248670 -->

    <owl:NamedIndividual rdf:about="http://purl.obolibrary.org/obo/GAZ_00248670">
        <obo:RO_0001025 rdf:resource="http://purl.obolibrary.org/obo/GAZ_00400063"/>
        <obo:IAO_0000115>A flood control mechanism located at the Chenab River near the city of Sialkot, Punjab, Pakistan. Constructed 1968.</obo:IAO_0000115>
        <oboInOwl:hasOBONamespace>GAZ</oboInOwl:hasOBONamespace>
        <oboInOwl:id>GAZ:00248670</oboInOwl:id>
        <rdfs:label>Marala Headworks</rdfs:label>
    </owl:NamedIndividual>
    


    <!-- http://purl.obolibrary.org/obo/GAZ_00248671 -->

    <owl:NamedIndividual rdf:about="http://purl.obolibrary.org/obo/GAZ_00248671">
        <obo:RO_0001025 rdf:resource="http://purl.obolibrary.org/obo/GAZ_00248628"/>
        <obo:RO_0001025 rdf:resource="http://purl.obolibrary.org/obo/GAZ_00253077"/>
        <obo:IAO_0000115>An impoundment located on the Indus river in the Punjab province of Pakistan. Completed 1958.</obo:IAO_0000115>
        <oboInOwl:hasOBONamespace>GAZ</oboInOwl:hasOBONamespace>
        <oboInOwl:id>GAZ:00248671</oboInOwl:id>
        <rdfs:label>Taunsa Barrage</rdfs:label>
    </owl:NamedIndividual>
    


    <!-- http://purl.obolibrary.org/obo/GAZ_00248672 -->

    <owl:NamedIndividual rdf:about="http://purl.obolibrary.org/obo/GAZ_00248672">
        <obo:RO_0001025 rdf:resource="http://purl.obolibrary.org/obo/GAZ_00148807"/>
        <obo:RO_0001025 rdf:resource="http://purl.obolibrary.org/obo/GAZ_00400077"/>
        <obo:IAO_0000115>A hydro engineering project. It is used to control water flow in the river. It is situated at Sutlej river near Hasilpur in Bahawalpur District.</obo:IAO_0000115>
        <oboInOwl:hasOBONamespace>GAZ</oboInOwl:hasOBONamespace>
        <oboInOwl:id>GAZ:00248672</oboInOwl:id>
        <rdfs:label>Head Islam</rdfs:label>
    </owl:NamedIndividual>
    


    <!-- http://purl.obolibrary.org/obo/GAZ_00248673 -->

    <owl:NamedIndividual rdf:about="http://purl.obolibrary.org/obo/GAZ_00248673">
        <obo:RO_0001025 rdf:resource="http://purl.obolibrary.org/obo/GAZ_00080536"/>
        <obo:IAO_0000115>A hydroelectric plant located on the river Chenab in the Punjab province of Pakistan. It is in Phalia Tehsil of Mandi Bahauddin District.</obo:IAO_0000115>
        <oboInOwl:hasOBONamespace>GAZ</oboInOwl:hasOBONamespace>
        <oboInOwl:id>GAZ:00248673</oboInOwl:id>
        <rdfs:label>Head Qadirabad</rdfs:label>
    </owl:NamedIndividual>
    


    <!-- http://purl.obolibrary.org/obo/GAZ_00248679 -->

    <owl:NamedIndividual rdf:about="http://purl.obolibrary.org/obo/GAZ_00248679">
        <obo:RO_0001025 rdf:resource="http://purl.obolibrary.org/obo/GAZ_00018578"/>
        <obo:IAO_0000115>A valley located in Astore District in the autonomous Pakistani regions of Gilgit-Baltistan. Adjoins the eastern side of mountain Nanga Parbat.</obo:IAO_0000115>
        <oboInOwl:hasOBONamespace>GAZ</oboInOwl:hasOBONamespace>
        <oboInOwl:id>GAZ:00248679</oboInOwl:id>
        <rdfs:label>Astore Valley</rdfs:label>
    </owl:NamedIndividual>
    


    <!-- http://purl.obolibrary.org/obo/GAZ_00248684 -->

    <owl:NamedIndividual rdf:about="http://purl.obolibrary.org/obo/GAZ_00248684">
        <obo:IAO_0000115>A river.</obo:IAO_0000115>
        <oboInOwl:hasOBONamespace>GAZ</oboInOwl:hasOBONamespace>
        <oboInOwl:id>GAZ:00248684</oboInOwl:id>
        <rdfs:label>Zanskar River</rdfs:label>
    </owl:NamedIndividual>
    


    <!-- http://purl.obolibrary.org/obo/GAZ_00248687 -->

    <owl:NamedIndividual rdf:about="http://purl.obolibrary.org/obo/GAZ_00248687">
        <obo:RO_0001025 rdf:resource="http://purl.obolibrary.org/obo/GAZ_00080415"/>
        <obo:IAO_0000115>A populated place. A city and the headquarters of Kulachi Tehsil of Dera Ismail Khan District in North-West Frontier Province, Pakistan.</obo:IAO_0000115>
        <oboInOwl:hasOBONamespace>GAZ</oboInOwl:hasOBONamespace>
        <oboInOwl:id>GAZ:00248687</oboInOwl:id>
        <rdfs:label>Kulachi</rdfs:label>
    </owl:NamedIndividual>
    


    <!-- http://purl.obolibrary.org/obo/GAZ_00248688 -->

    <owl:NamedIndividual rdf:about="http://purl.obolibrary.org/obo/GAZ_00248688">
        <rdf:type rdf:resource="http://purl.obolibrary.org/obo/ENVO_00000074"/>
        <obo:RO_0001025 rdf:resource="http://purl.obolibrary.org/obo/GAZ_00248628"/>
        <obo:RO_0001025 rdf:resource="http://purl.obolibrary.org/obo/GAZ_00248689"/>
        <obo:IAO_0000115>A barrage. Located 25 km southwest of Mianwali, on the Mianwali to Dera Ismail Khan road, Punjab Province. Completed 1971.</obo:IAO_0000115>
        <oboInOwl:hasOBONamespace>GAZ</oboInOwl:hasOBONamespace>
        <oboInOwl:id>GAZ:00248688</oboInOwl:id>
        <rdfs:label>Chashma Barrage</rdfs:label>
    </owl:NamedIndividual>
    


    <!-- http://purl.obolibrary.org/obo/GAZ_00248689 -->

    <owl:NamedIndividual rdf:about="http://purl.obolibrary.org/obo/GAZ_00248689">
        <obo:RO_0001025 rdf:resource="http://purl.obolibrary.org/obo/GAZ_00400056"/>
        <obo:IAO_0000115>A populated place.</obo:IAO_0000115>
        <oboInOwl:hasOBONamespace>GAZ</oboInOwl:hasOBONamespace>
        <oboInOwl:id>GAZ:00248689</oboInOwl:id>
        <rdfs:label>Chashma Colony</rdfs:label>
    </owl:NamedIndividual>
    


    <!-- http://purl.obolibrary.org/obo/GAZ_00248691 -->

    <owl:NamedIndividual rdf:about="http://purl.obolibrary.org/obo/GAZ_00248691">
        <obo:RO_0001025 rdf:resource="http://purl.obolibrary.org/obo/GAZ_00248628"/>
        <obo:RO_0001025 rdf:resource="http://purl.obolibrary.org/obo/GAZ_00400041"/>
        <obo:IAO_0000115>A large dam on the Indus River in Pakistan. It is located in Haripur district of Hazara Division of North-West Frontier Province about 50 km northwest of Islamabad. Constructed 1968-1974.</obo:IAO_0000115>
        <oboInOwl:hasOBONamespace>GAZ</oboInOwl:hasOBONamespace>
        <oboInOwl:id>GAZ:00248691</oboInOwl:id>
        <rdfs:label>Tarbela Dam</rdfs:label>
    </owl:NamedIndividual>
    


    <!-- http://purl.obolibrary.org/obo/GAZ_00248693 -->

    <owl:NamedIndividual rdf:about="http://purl.obolibrary.org/obo/GAZ_00248693">
        <obo:IAO_0000115>A large water storage reservoir. Located on the Hub River on the arid plains north of Karachi. It is located on the provincial border between Balochistan and Sindh, Pakistan. Impounds Hub Reservoir. Constructed 1981.</obo:IAO_0000115>
        <oboInOwl:hasOBONamespace>GAZ</oboInOwl:hasOBONamespace>
        <oboInOwl:id>GAZ:00248693</oboInOwl:id>
        <rdfs:label>Hub Dam</rdfs:label>
    </owl:NamedIndividual>
    


    <!-- http://purl.obolibrary.org/obo/GAZ_00248694 -->

    <owl:NamedIndividual rdf:about="http://purl.obolibrary.org/obo/GAZ_00248694">
        <obo:IAO_0000115>A reservoir. Impounded by the Hub Dam. Constructed 1981. A Ramsar Site.</obo:IAO_0000115>
        <oboInOwl:hasOBONamespace>GAZ</oboInOwl:hasOBONamespace>
        <oboInOwl:id>GAZ:00248694</oboInOwl:id>
        <rdfs:label>Hub Reservoir</rdfs:label>
    </owl:NamedIndividual>
    


    <!-- http://purl.obolibrary.org/obo/GAZ_00248697 -->

    <owl:NamedIndividual rdf:about="http://purl.obolibrary.org/obo/GAZ_00248697">
        <obo:RO_0001025 rdf:resource="http://purl.obolibrary.org/obo/GAZ_00005249"/>
        <obo:IAO_0000115>A plateau in the province of Punjab, Pakistan. It is bounded on the east by the Jhelum River, on the west by the Indus River, on the north by the Kala Chitta Range and the Margalla Hills, and on the south by the Salt Range.</obo:IAO_0000115>
        <oboInOwl:hasOBONamespace>GAZ</oboInOwl:hasOBONamespace>
        <oboInOwl:id>GAZ:00248697</oboInOwl:id>
        <rdfs:label>Pothohar Plateau</rdfs:label>
    </owl:NamedIndividual>
    


    <!-- http://purl.obolibrary.org/obo/GAZ_00248698 -->

    <owl:NamedIndividual rdf:about="http://purl.obolibrary.org/obo/GAZ_00248698">
        <obo:IAO_0000115>A dam.</obo:IAO_0000115>
        <oboInOwl:hasOBONamespace>GAZ</oboInOwl:hasOBONamespace>
        <oboInOwl:id>GAZ:00248698</oboInOwl:id>
        <rdfs:label>Simblee Dam</rdfs:label>
    </owl:NamedIndividual>
    


    <!-- http://purl.obolibrary.org/obo/GAZ_00248709 -->

    <owl:NamedIndividual rdf:about="http://purl.obolibrary.org/obo/GAZ_00248709">
        <obo:IAO_0000115>A mountain range in the Indian state of Jammu and Kashmir that separates Zanskar from Ladakh.</obo:IAO_0000115>
        <oboInOwl:hasOBONamespace>GAZ</oboInOwl:hasOBONamespace>
        <oboInOwl:id>GAZ:00248709</oboInOwl:id>
        <rdfs:label>Zanskar Range</rdfs:label>
    </owl:NamedIndividual>
    


    <!-- http://purl.obolibrary.org/obo/GAZ_00248712 -->

    <owl:NamedIndividual rdf:about="http://purl.obolibrary.org/obo/GAZ_00248712">
        <obo:IAO_0000115>A headwater of the Zanskar River. A river of Jammu and Kashmir in northern India. It flows through the Zanskar region of the state of Ladakh.</obo:IAO_0000115>
        <oboInOwl:hasOBONamespace>GAZ</oboInOwl:hasOBONamespace>
        <oboInOwl:id>GAZ:00248712</oboInOwl:id>
        <rdfs:label>Tsarap River</rdfs:label>
    </owl:NamedIndividual>
    


    <!-- http://purl.obolibrary.org/obo/GAZ_00248717 -->

    <owl:NamedIndividual rdf:about="http://purl.obolibrary.org/obo/GAZ_00248717">
        <obo:IAO_0000115>A river that originates at the Thamsar Glacier in the Dhauladhar range of the Himalayas, flows through the Uhl valley crossing Bada Gran and Barot, both villages in the Uhl valley. In the lower part of its course, it is also known as Tiun Nala and the Uhl valley is known as Chohar valley. After passing the Chohar valley, Uhl meets the Beas river 5 km downstream from Pandoh.</obo:IAO_0000115>
        <oboInOwl:hasOBONamespace>GAZ</oboInOwl:hasOBONamespace>
        <oboInOwl:id>GAZ:00248717</oboInOwl:id>
        <rdfs:label>Uhl River</rdfs:label>
    </owl:NamedIndividual>
    


    <!-- http://purl.obolibrary.org/obo/GAZ_00248721 -->

    <owl:NamedIndividual rdf:about="http://purl.obolibrary.org/obo/GAZ_00248721">
        <obo:RO_0001025 rdf:resource="http://purl.obolibrary.org/obo/GAZ_00400046"/>
        <obo:IAO_0000115>A river located in Bannu District, North-West Frontier Province, Pakistan.</obo:IAO_0000115>
        <oboInOwl:hasOBONamespace>GAZ</oboInOwl:hasOBONamespace>
        <oboInOwl:id>GAZ:00248721</oboInOwl:id>
        <rdfs:label>Gambila River</rdfs:label>
    </owl:NamedIndividual>
    


    <!-- http://purl.obolibrary.org/obo/GAZ_00248723 -->

    <owl:NamedIndividual rdf:about="http://purl.obolibrary.org/obo/GAZ_00248723">
        <rdf:type rdf:resource="http://purl.obolibrary.org/obo/ENVO_00000856"/>
        <obo:RO_0001025 rdf:resource="http://purl.obolibrary.org/obo/GAZ_00018583"/>
        <obo:IAO_0000115>A populated place. A town near to the Gilgit Valley in the Northern Areas of Pakistan. The town is located in Gilgit District and was the capital of the former State of Nagar.</obo:IAO_0000115>
        <oboInOwl:hasOBONamespace>GAZ</oboInOwl:hasOBONamespace>
        <oboInOwl:id>GAZ:00248723</oboInOwl:id>
        <rdfs:label>Nagar</rdfs:label>
    </owl:NamedIndividual>
    


    <!-- http://purl.obolibrary.org/obo/GAZ_00248724 -->

    <owl:NamedIndividual rdf:about="http://purl.obolibrary.org/obo/GAZ_00248724">
        <obo:RO_0001025 rdf:resource="http://purl.obolibrary.org/obo/GAZ_00005256"/>
        <obo:RO_0001025 rdf:resource="http://purl.obolibrary.org/obo/GAZ_00056909"/>
        <obo:IAO_0000115>A 49 km long glacier in the Karakoram Mountains of the (Northern Areas, Pakistan) which meets the 63 km long Biafo Glacier at the Hispar La (Pass) at an altitude of 5,128 m to create the world&apos;s longest glacial system outside of the polar regions.</obo:IAO_0000115>
        <oboInOwl:hasOBONamespace>GAZ</oboInOwl:hasOBONamespace>
        <oboInOwl:id>GAZ:00248724</oboInOwl:id>
        <rdfs:label>Hispar Glacier</rdfs:label>
    </owl:NamedIndividual>
    


    <!-- http://purl.obolibrary.org/obo/GAZ_00248725 -->

    <owl:NamedIndividual rdf:about="http://purl.obolibrary.org/obo/GAZ_00248725">
        <obo:RO_0001025 rdf:resource="http://purl.obolibrary.org/obo/GAZ_00005256"/>
        <obo:IAO_0000115>A 63 km long glacier in the Karakoram Mountains of the Northern Areas, Pakistan which meets the 49 km long Hispar Glacier at an altitude of 5,128 m at Hispar La (Pass) to create the world&apos;s longest glacial system outside the polar regions.</obo:IAO_0000115>
        <oboInOwl:hasOBONamespace>GAZ</oboInOwl:hasOBONamespace>
        <oboInOwl:id>GAZ:00248725</oboInOwl:id>
        <rdfs:label>Biafo Glacier</rdfs:label>
    </owl:NamedIndividual>
    


    <!-- http://purl.obolibrary.org/obo/GAZ_00248726 -->

    <owl:NamedIndividual rdf:about="http://purl.obolibrary.org/obo/GAZ_00248726">
        <obo:RO_0001025 rdf:resource="http://purl.obolibrary.org/obo/GAZ_00018579"/>
        <obo:IAO_0000115>A 62 km long, glacier. It is located in Baltistan, in the Gilgit-Baltistan region of Pakistan, and runs through part of the Karakoram mountain range. The Baltoro Muztagh lies to the north and east of the glacier, while the Masherbrum Mountains lie to the south. The glacier gives rise to the Shigar River.</obo:IAO_0000115>
        <oboInOwl:hasOBONamespace>GAZ</oboInOwl:hasOBONamespace>
        <oboInOwl:id>GAZ:00248726</oboInOwl:id>
        <rdfs:label>Baltoro Glacier</rdfs:label>
    </owl:NamedIndividual>
    


    <!-- http://purl.obolibrary.org/obo/GAZ_00248732 -->

    <owl:NamedIndividual rdf:about="http://purl.obolibrary.org/obo/GAZ_00248732">
        <obo:IAO_0000115>A glacier in the autonomous region Xinjiang of China, in the Karakoram mountain range of the Himalayas. It lies north of the Baltoro Muztagh range.</obo:IAO_0000115>
        <oboInOwl:hasOBONamespace>GAZ</oboInOwl:hasOBONamespace>
        <oboInOwl:id>GAZ:00248732</oboInOwl:id>
        <rdfs:label>Sarpo Laggo Glacier</rdfs:label>
    </owl:NamedIndividual>
    


    <!-- http://purl.obolibrary.org/obo/GAZ_00248733 -->

    <owl:NamedIndividual rdf:about="http://purl.obolibrary.org/obo/GAZ_00248733">
        <rdf:type rdf:resource="http://purl.obolibrary.org/obo/ENVO_00000100"/>
        <obo:RO_0001025 rdf:resource="http://purl.obolibrary.org/obo/GAZ_00005257"/>
        <obo:IAO_0000115>A Himalayan gorge in Azad Kashmir, Pakistan along which the Neelum River flows.</obo:IAO_0000115>
        <oboInOwl:hasOBONamespace>GAZ</oboInOwl:hasOBONamespace>
        <oboInOwl:id>GAZ:00248733</oboInOwl:id>
        <rdfs:label>Neelum Valley</rdfs:label>
    </owl:NamedIndividual>
    


    <!-- http://purl.obolibrary.org/obo/GAZ_00248735 -->

    <owl:NamedIndividual rdf:about="http://purl.obolibrary.org/obo/GAZ_00248735">
        <obo:RO_0001025 rdf:resource="http://purl.obolibrary.org/obo/GAZ_00400032"/>
        <obo:IAO_0000115>A valley in the upper reaches of the Swat River in Swat, in the North-West Frontier Province (NWFP) of Pakistan.</obo:IAO_0000115>
        <oboInOwl:hasOBONamespace>GAZ</oboInOwl:hasOBONamespace>
        <oboInOwl:id>GAZ:00248735</oboInOwl:id>
        <rdfs:label>Kalam Valley</rdfs:label>
    </owl:NamedIndividual>
    


    <!-- http://purl.obolibrary.org/obo/GAZ_00248736 -->

    <owl:NamedIndividual rdf:about="http://purl.obolibrary.org/obo/GAZ_00248736">
        <rdf:type rdf:resource="http://purl.obolibrary.org/obo/ENVO_00000856"/>
        <obo:RO_0001025 rdf:resource="http://purl.obolibrary.org/obo/GAZ_00080408"/>
        <obo:IAO_0000115>A populated place. A town and headquarters of Charsadda District, in the North-West Frontier Province of Pakistan.</obo:IAO_0000115>
        <oboInOwl:hasOBONamespace>GAZ</oboInOwl:hasOBONamespace>
        <oboInOwl:id>GAZ:00248736</oboInOwl:id>
        <rdfs:label>Charsadda</rdfs:label>
    </owl:NamedIndividual>
    


    <!-- http://purl.obolibrary.org/obo/GAZ_00248743 -->

    <owl:NamedIndividual rdf:about="http://purl.obolibrary.org/obo/GAZ_00248743">
        <obo:IAO_0000115>A river is located in Afghanistan.</obo:IAO_0000115>
        <oboInOwl:hasOBONamespace>GAZ</oboInOwl:hasOBONamespace>
        <oboInOwl:id>GAZ:00248743</oboInOwl:id>
        <rdfs:label>Peche River</rdfs:label>
    </owl:NamedIndividual>
    


    <!-- http://purl.obolibrary.org/obo/GAZ_00248745 -->

    <owl:NamedIndividual rdf:about="http://purl.obolibrary.org/obo/GAZ_00248745">
        <obo:RO_0001025 rdf:resource="http://purl.obolibrary.org/obo/GAZ_00057376"/>
        <obo:IAO_0000115>A glacier in the Great Himalaya subrange of Himalayas. It starts north of an unnamed 6,326 m high peak and flows northeastward, north of Laila Peak (Rupal Valley) and south of Nanga Parbat&apos;s many peaks. The meltwater from the glacier forms Rupal River.</obo:IAO_0000115>
        <oboInOwl:hasOBONamespace>GAZ</oboInOwl:hasOBONamespace>
        <oboInOwl:id>GAZ:00248745</oboInOwl:id>
        <rdfs:label>Rupal Glacier</rdfs:label>
    </owl:NamedIndividual>
    


    <!-- http://purl.obolibrary.org/obo/GAZ_00248746 -->

    <owl:NamedIndividual rdf:about="http://purl.obolibrary.org/obo/GAZ_00248746">
        <obo:RO_0001025 rdf:resource="http://purl.obolibrary.org/obo/GAZ_00018578"/>
        <obo:IAO_0000115>A valley located in the Astore District of Pakistan&apos;s Gilgit-Baltistan region.</obo:IAO_0000115>
        <oboInOwl:hasOBONamespace>GAZ</oboInOwl:hasOBONamespace>
        <oboInOwl:id>GAZ:00248746</oboInOwl:id>
        <rdfs:label>Rupal Valley</rdfs:label>
    </owl:NamedIndividual>
    


    <!-- http://purl.obolibrary.org/obo/GAZ_00248765 -->

    <owl:NamedIndividual rdf:about="http://purl.obolibrary.org/obo/GAZ_00248765">
        <obo:RO_0001025 rdf:resource="http://purl.obolibrary.org/obo/GAZ_00148807"/>
        <obo:IAO_0000115>A water storage reservoir. Located in Amritsar District, 55 km south of Amritsar, Punjab. Formed by the construction of a barrage at Harike at the confluence of the Sutlej and Beas Rivers. The lake forms the headworks of the Rajasthan, Ferozapur and Makku feeder canals. Constructed 1953.</obo:IAO_0000115>
        <oboInOwl:hasOBONamespace>GAZ</oboInOwl:hasOBONamespace>
        <oboInOwl:id>GAZ:00248765</oboInOwl:id>
        <rdfs:label>Harike Lake</rdfs:label>
    </owl:NamedIndividual>
    


    <!-- http://purl.obolibrary.org/obo/GAZ_00248766 -->

    <owl:NamedIndividual rdf:about="http://purl.obolibrary.org/obo/GAZ_00248766">
        <obo:RO_0001025 rdf:resource="http://purl.obolibrary.org/obo/GAZ_00148807"/>
        <obo:IAO_0000115>A dam. Impounds Harike Lake. Constructed 1953.</obo:IAO_0000115>
        <oboInOwl:hasOBONamespace>GAZ</oboInOwl:hasOBONamespace>
        <oboInOwl:id>GAZ:00248766</oboInOwl:id>
        <rdfs:label>Harike Barrage</rdfs:label>
    </owl:NamedIndividual>
    


    <!-- http://purl.obolibrary.org/obo/GAZ_00248767 -->

    <owl:NamedIndividual rdf:about="http://purl.obolibrary.org/obo/GAZ_00248767">
        <oboInOwl:hasOBONamespace>GAZ</oboInOwl:hasOBONamespace>
        <oboInOwl:id>GAZ:00248767</oboInOwl:id>
        <rdfs:label>Rajasthan Main Canal</rdfs:label>
    </owl:NamedIndividual>
    


    <!-- http://purl.obolibrary.org/obo/GAZ_00248768 -->

    <owl:NamedIndividual rdf:about="http://purl.obolibrary.org/obo/GAZ_00248768">
        <oboInOwl:hasOBONamespace>GAZ</oboInOwl:hasOBONamespace>
        <oboInOwl:id>GAZ:00248768</oboInOwl:id>
        <rdfs:label>Rajasthan Feeder Canal</rdfs:label>
    </owl:NamedIndividual>
    


    <!-- http://purl.obolibrary.org/obo/GAZ_00248809 -->

    <owl:NamedIndividual rdf:about="http://purl.obolibrary.org/obo/GAZ_00248809">
        <obo:RO_0001025 rdf:resource="http://purl.obolibrary.org/obo/GAZ_00248810"/>
        <obo:IAO_0000115>A wetland in the Uttarakhand-Himachal Pradesh border region in Doon Valley, (Dehradun District), northern India, situated at the confluence of the Yamuna Canal and the Assan River and about 11 km from Dak Pathar, and 28 km southwest of Dehradun.</obo:IAO_0000115>
        <oboInOwl:hasOBONamespace>GAZ</oboInOwl:hasOBONamespace>
        <oboInOwl:id>GAZ:00248809</oboInOwl:id>
        <rdfs:label>Assan Barrage</rdfs:label>
    </owl:NamedIndividual>
    


    <!-- http://purl.obolibrary.org/obo/GAZ_00248810 -->

    <owl:NamedIndividual rdf:about="http://purl.obolibrary.org/obo/GAZ_00248810">
        <obo:RO_0001025 rdf:resource="http://purl.obolibrary.org/obo/GAZ_00058368"/>
        <obo:IAO_0000115>A valley located in Sivalik Hills in Uttarakhand, India, home to the capital of Indian state of Uttarakhand, Dehradun.</obo:IAO_0000115>
        <oboInOwl:hasOBONamespace>GAZ</oboInOwl:hasOBONamespace>
        <oboInOwl:id>GAZ:00248810</oboInOwl:id>
        <rdfs:label>Doon Valley</rdfs:label>
    </owl:NamedIndividual>
    


    <!-- http://purl.obolibrary.org/obo/GAZ_00248849 -->

    <owl:NamedIndividual rdf:about="http://purl.obolibrary.org/obo/GAZ_00248849">
        <obo:IAO_0000115>A river flowing in Bhind District of Madhya Pradesh in central India.</obo:IAO_0000115>
        <oboInOwl:hasOBONamespace>GAZ</oboInOwl:hasOBONamespace>
        <oboInOwl:id>GAZ:00248849</oboInOwl:id>
        <rdfs:label>Pahuj River</rdfs:label>
    </owl:NamedIndividual>
    


    <!-- http://purl.obolibrary.org/obo/GAZ_00248855 -->

    <owl:NamedIndividual rdf:about="http://purl.obolibrary.org/obo/GAZ_00248855">
        <rdf:type rdf:resource="http://purl.obolibrary.org/obo/ENVO_00000074"/>
        <obo:IAO_0000115>A barrage.</obo:IAO_0000115>
        <oboInOwl:hasOBONamespace>GAZ</oboInOwl:hasOBONamespace>
        <oboInOwl:id>GAZ:00248855</oboInOwl:id>
        <rdfs:label>Okhla Barrage</rdfs:label>
    </owl:NamedIndividual>
    


    <!-- http://purl.obolibrary.org/obo/GAZ_00248865 -->

    <owl:NamedIndividual rdf:about="http://purl.obolibrary.org/obo/GAZ_00248865">
        <obo:IAO_0000115>An island within the Rann of Kutch.</obo:IAO_0000115>
        <oboInOwl:hasOBONamespace>GAZ</oboInOwl:hasOBONamespace>
        <oboInOwl:id>GAZ:00248865</oboInOwl:id>
        <rdfs:label>Pachham Island</rdfs:label>
    </owl:NamedIndividual>
    


    <!-- http://purl.obolibrary.org/obo/GAZ_00248868 -->

    <owl:NamedIndividual rdf:about="http://purl.obolibrary.org/obo/GAZ_00248868">
        <obo:IAO_0000115>A protected area. Established 1986-02.</obo:IAO_0000115>
        <oboInOwl:hasOBONamespace>GAZ</oboInOwl:hasOBONamespace>
        <oboInOwl:id>GAZ:00248868</oboInOwl:id>
        <rdfs:label>Kutch Desert Wildlife Sanctuary</rdfs:label>
    </owl:NamedIndividual>
    


    <!-- http://purl.obolibrary.org/obo/GAZ_00248873 -->

    <owl:NamedIndividual rdf:about="http://purl.obolibrary.org/obo/GAZ_00248873">
        <obo:IAO_0000115>A protected area.</obo:IAO_0000115>
        <oboInOwl:hasOBONamespace>GAZ</oboInOwl:hasOBONamespace>
        <oboInOwl:id>GAZ:00248873</oboInOwl:id>
        <rdfs:label>Kutch Bustard Sanctuary</rdfs:label>
    </owl:NamedIndividual>
    


    <!-- http://purl.obolibrary.org/obo/GAZ_00248874 -->

    <owl:NamedIndividual rdf:about="http://purl.obolibrary.org/obo/GAZ_00248874">
        <obo:IAO_0000115>A protected area of arid grassland ecosystem on the outer southern edge of the desert of the marshy salt flats of Rann of Kutch in Kutch District, Gujarat State, India.</obo:IAO_0000115>
        <oboInOwl:hasOBONamespace>GAZ</oboInOwl:hasOBONamespace>
        <oboInOwl:id>GAZ:00248874</oboInOwl:id>
        <rdfs:label>Banni Grasslands Reserve</rdfs:label>
    </owl:NamedIndividual>
    


    <!-- http://purl.obolibrary.org/obo/GAZ_00248875 -->

    <owl:NamedIndividual rdf:about="http://purl.obolibrary.org/obo/GAZ_00248875">
        <obo:IAO_0000115>A protected area located on the edge of arid Banni grasslands and the marshy salt flats of the Rann of Kutch in Kutch District, Gujarat State in India.</obo:IAO_0000115>
        <oboInOwl:hasOBONamespace>GAZ</oboInOwl:hasOBONamespace>
        <oboInOwl:id>GAZ:00248875</oboInOwl:id>
        <rdfs:label>Chari-Dhand Wetland Conservation Reserve</rdfs:label>
    </owl:NamedIndividual>
    


    <!-- http://purl.obolibrary.org/obo/GAZ_00248876 -->

    <owl:NamedIndividual rdf:about="http://purl.obolibrary.org/obo/GAZ_00248876">
        <obo:RO_0001025 rdf:resource="http://purl.obolibrary.org/obo/GAZ_00400085"/>
        <obo:IAO_0000115>A protected area located in Badin District, Sindh, Pakistan.</obo:IAO_0000115>
        <oboInOwl:hasOBONamespace>GAZ</oboInOwl:hasOBONamespace>
        <oboInOwl:id>GAZ:00248876</oboInOwl:id>
        <rdfs:label>Rann of Kutch Wildlife Sanctuary</rdfs:label>
    </owl:NamedIndividual>
    


    <!-- http://purl.obolibrary.org/obo/GAZ_00251825 -->

    <owl:NamedIndividual rdf:about="http://purl.obolibrary.org/obo/GAZ_00251825">
        <obo:RO_0001025 rdf:resource="http://purl.obolibrary.org/obo/GAZ_00018579"/>
        <obo:IAO_0000115>A high plateau of moorland and swamp with numerous small lakes and ponds, in the upper drainage of the Indus River at the northwestern extremity of the Great Himalayan Range.</obo:IAO_0000115>
        <oboInOwl:hasOBONamespace>GAZ</oboInOwl:hasOBONamespace>
        <oboInOwl:id>GAZ:00251825</oboInOwl:id>
        <rdfs:label>Deosai Plateau</rdfs:label>
    </owl:NamedIndividual>
    


    <!-- http://purl.obolibrary.org/obo/GAZ_00253060 -->

    <owl:NamedIndividual rdf:about="http://purl.obolibrary.org/obo/GAZ_00253060">
        <obo:RO_0001025 rdf:resource="http://purl.obolibrary.org/obo/GAZ_00248628"/>
        <obo:RO_0001025 rdf:resource="http://purl.obolibrary.org/obo/GAZ_00400041"/>
        <obo:IAO_0000115>A reservoir. Impounded by Tarbela Dam. Completed 1974.</obo:IAO_0000115>
        <oboInOwl:hasOBONamespace>GAZ</oboInOwl:hasOBONamespace>
        <oboInOwl:id>GAZ:00253060</oboInOwl:id>
        <rdfs:label>Tarbela Reservoir</rdfs:label>
    </owl:NamedIndividual>
    


    <!-- http://purl.obolibrary.org/obo/GAZ_00253061 -->

    <owl:NamedIndividual rdf:about="http://purl.obolibrary.org/obo/GAZ_00253061">
        <obo:RO_0001025 rdf:resource="http://purl.obolibrary.org/obo/GAZ_00400044"/>
        <obo:IAO_0000115>A small freshwater reservoir. Located east of the village of Barh, 7 km west of Kohat.</obo:IAO_0000115>
        <oboInOwl:hasOBONamespace>GAZ</oboInOwl:hasOBONamespace>
        <oboInOwl:id>GAZ:00253061</oboInOwl:id>
        <rdfs:label>Tanda Dam Reservoir</rdfs:label>
    </owl:NamedIndividual>
    


    <!-- http://purl.obolibrary.org/obo/GAZ_00253063 -->

    <owl:NamedIndividual rdf:about="http://purl.obolibrary.org/obo/GAZ_00253063">
        <obo:RO_0001025 rdf:resource="http://purl.obolibrary.org/obo/GAZ_00400046"/>
        <obo:IAO_0000115>A protected area. Includes a shallow, fresh to brackish seepage lagoon and extensive marshy area formed at the junction of Gambilla and Kurram rivers. Established 1976.</obo:IAO_0000115>
        <oboInOwl:hasOBONamespace>GAZ</oboInOwl:hasOBONamespace>
        <oboInOwl:id>GAZ:00253063</oboInOwl:id>
        <rdfs:label>Thanedar Wala Game Reserve</rdfs:label>
    </owl:NamedIndividual>
    


    <!-- http://purl.obolibrary.org/obo/GAZ_00253064 -->

    <owl:NamedIndividual rdf:about="http://purl.obolibrary.org/obo/GAZ_00253064">
        <obo:RO_0001025 rdf:resource="http://purl.obolibrary.org/obo/GAZ_00400046"/>
        <obo:IAO_0000115>A flood control dam and water storage reservoir near the Kurram River about ten km west of Bannu. The reservoir is fed by a canal from the Kurram River.</obo:IAO_0000115>
        <oboInOwl:hasOBONamespace>GAZ</oboInOwl:hasOBONamespace>
        <oboInOwl:id>GAZ:00253064</oboInOwl:id>
        <rdfs:label>Baran Dam</rdfs:label>
    </owl:NamedIndividual>
    


    <!-- http://purl.obolibrary.org/obo/GAZ_00253065 -->

    <owl:NamedIndividual rdf:about="http://purl.obolibrary.org/obo/GAZ_00253065">
        <obo:IAO_0000115>A dead arm of the Kurram River on the west bank of the river about 20 km northwest of Lakki, in a region of irrigated fields and small villages.</obo:IAO_0000115>
        <oboInOwl:hasOBONamespace>GAZ</oboInOwl:hasOBONamespace>
        <oboInOwl:id>GAZ:00253065</oboInOwl:id>
        <rdfs:label>Malugul Dhand</rdfs:label>
    </owl:NamedIndividual>
    


    <!-- http://purl.obolibrary.org/obo/GAZ_00253066 -->

    <owl:NamedIndividual rdf:about="http://purl.obolibrary.org/obo/GAZ_00253066">
        <obo:RO_0001025 rdf:resource="http://purl.obolibrary.org/obo/GAZ_00248689"/>
        <obo:IAO_0000115>A protected area. Established 1972.</obo:IAO_0000115>
        <oboInOwl:hasOBONamespace>GAZ</oboInOwl:hasOBONamespace>
        <oboInOwl:id>GAZ:00253066</oboInOwl:id>
        <rdfs:label>Chashma Lake Wildlife Sanctuary</rdfs:label>
    </owl:NamedIndividual>
    


    <!-- http://purl.obolibrary.org/obo/GAZ_00253067 -->

    <owl:NamedIndividual rdf:about="http://purl.obolibrary.org/obo/GAZ_00253067">
        <obo:RO_0001025 rdf:resource="http://purl.obolibrary.org/obo/GAZ_00400056"/>
        <obo:IAO_0000115>A protected area. Established 1970.</obo:IAO_0000115>
        <oboInOwl:hasOBONamespace>GAZ</oboInOwl:hasOBONamespace>
        <oboInOwl:id>GAZ:00253067</oboInOwl:id>
        <rdfs:label>Namal Lake Wildlife Sanctuary</rdfs:label>
    </owl:NamedIndividual>
    


    <!-- http://purl.obolibrary.org/obo/GAZ_00253068 -->

    <owl:NamedIndividual rdf:about="http://purl.obolibrary.org/obo/GAZ_00253068">
        <obo:IAO_0000115>A deep freshwater reservoir on the Jhelum River, spanning the border between Punjab Province and Azad Kashmir, in the foothills of the Pir Panjal Range. Impounded by Mangla Dam. Completed 1967.</obo:IAO_0000115>
        <oboInOwl:hasOBONamespace>GAZ</oboInOwl:hasOBONamespace>
        <oboInOwl:id>GAZ:00253068</oboInOwl:id>
        <rdfs:label>Mangla Reservoir</rdfs:label>
    </owl:NamedIndividual>
    


    <!-- http://purl.obolibrary.org/obo/GAZ_00253069 -->

    <owl:NamedIndividual rdf:about="http://purl.obolibrary.org/obo/GAZ_00253069">
        <obo:RO_0001025 rdf:resource="http://purl.obolibrary.org/obo/GAZ_00056904"/>
        <obo:RO_0001025 rdf:resource="http://purl.obolibrary.org/obo/GAZ_00400068"/>
        <obo:IAO_0000115>A small brackish to saline lake.</obo:IAO_0000115>
        <oboInOwl:hasOBONamespace>GAZ</oboInOwl:hasOBONamespace>
        <oboInOwl:id>GAZ:00253069</oboInOwl:id>
        <rdfs:label>Jahlar Lake</rdfs:label>
    </owl:NamedIndividual>
    


    <!-- http://purl.obolibrary.org/obo/GAZ_00253070 -->

    <owl:NamedIndividual rdf:about="http://purl.obolibrary.org/obo/GAZ_00253070">
        <obo:RO_0001025 rdf:resource="http://purl.obolibrary.org/obo/GAZ_00058477"/>
        <obo:RO_0001025 rdf:resource="http://purl.obolibrary.org/obo/GAZ_00400068"/>
        <obo:IAO_0000115>A protected area. Established 1967.</obo:IAO_0000115>
        <oboInOwl:hasOBONamespace>GAZ</oboInOwl:hasOBONamespace>
        <oboInOwl:id>GAZ:00253070</oboInOwl:id>
        <rdfs:label>Khabbaki Lake Wildlife Sanctuary</rdfs:label>
    </owl:NamedIndividual>
    


    <!-- http://purl.obolibrary.org/obo/GAZ_00253071 -->

    <owl:NamedIndividual rdf:about="http://purl.obolibrary.org/obo/GAZ_00253071">
        <obo:RO_0001025 rdf:resource="http://purl.obolibrary.org/obo/GAZ_00253072"/>
        <obo:IAO_0000115>A water storage reservoir. Located on the Jhelum River, 30 km downstream from Jhelum and 52 km WNW of Gujrat, Punjab Province.</obo:IAO_0000115>
        <oboInOwl:hasOBONamespace>GAZ</oboInOwl:hasOBONamespace>
        <oboInOwl:id>GAZ:00253071</oboInOwl:id>
        <rdfs:label>Rasul Barrage</rdfs:label>
    </owl:NamedIndividual>
    


    <!-- http://purl.obolibrary.org/obo/GAZ_00253072 -->

    <owl:NamedIndividual rdf:about="http://purl.obolibrary.org/obo/GAZ_00253072">
        <obo:RO_0001025 rdf:resource="http://purl.obolibrary.org/obo/GAZ_00400071"/>
        <obo:IAO_0000115>A protected area. Established 1974.</obo:IAO_0000115>
        <oboInOwl:hasOBONamespace>GAZ</oboInOwl:hasOBONamespace>
        <oboInOwl:id>GAZ:00253072</oboInOwl:id>
        <rdfs:label>Rasool Barrage Wildlife Sanctuary</rdfs:label>
    </owl:NamedIndividual>
    


    <!-- http://purl.obolibrary.org/obo/GAZ_00253073 -->

    <owl:NamedIndividual rdf:about="http://purl.obolibrary.org/obo/GAZ_00253073">
        <obo:RO_0001025 rdf:resource="http://purl.obolibrary.org/obo/GAZ_00400063"/>
        <obo:IAO_0000115>A protected area. Established 1987.</obo:IAO_0000115>
        <oboInOwl:hasOBONamespace>GAZ</oboInOwl:hasOBONamespace>
        <oboInOwl:id>GAZ:00253073</oboInOwl:id>
        <rdfs:label>Bajwat Game Reserve</rdfs:label>
    </owl:NamedIndividual>
    


    <!-- http://purl.obolibrary.org/obo/GAZ_00253074 -->

    <owl:NamedIndividual rdf:about="http://purl.obolibrary.org/obo/GAZ_00253074">
        <obo:RO_0001025 rdf:resource="http://purl.obolibrary.org/obo/GAZ_00400070"/>
        <obo:IAO_0000115>A shallow brackish lake and associated marshes on the plains between the Sutlej and Ravi Rivers. Located 2 km northeast of Chunian, Kasur District.</obo:IAO_0000115>
        <oboInOwl:hasOBONamespace>GAZ</oboInOwl:hasOBONamespace>
        <oboInOwl:id>GAZ:00253074</oboInOwl:id>
        <rdfs:label>Ghamaghar Lake</rdfs:label>
    </owl:NamedIndividual>
    


    <!-- http://purl.obolibrary.org/obo/GAZ_00253075 -->

    <owl:NamedIndividual rdf:about="http://purl.obolibrary.org/obo/GAZ_00253075">
        <obo:RO_0001025 rdf:resource="http://purl.obolibrary.org/obo/GAZ_00253076"/>
        <obo:IAO_0000115>A shallow brackish to saline lake. Located on the plains to the south of the Ravi River, 20 km northeast of Okara, Okara District, Punjab Province.</obo:IAO_0000115>
        <oboInOwl:hasOBONamespace>GAZ</oboInOwl:hasOBONamespace>
        <oboInOwl:id>GAZ:00253075</oboInOwl:id>
        <rdfs:label>Kharal Lake</rdfs:label>
    </owl:NamedIndividual>
    


    <!-- http://purl.obolibrary.org/obo/GAZ_00253076 -->

    <owl:NamedIndividual rdf:about="http://purl.obolibrary.org/obo/GAZ_00253076">
        <obo:RO_0001025 rdf:resource="http://purl.obolibrary.org/obo/GAZ_00400055"/>
        <obo:IAO_0000115>A protected area. Established 1971.</obo:IAO_0000115>
        <oboInOwl:hasOBONamespace>GAZ</oboInOwl:hasOBONamespace>
        <oboInOwl:id>GAZ:00253076</oboInOwl:id>
        <rdfs:label>Kharal Lake Wildlife Sanctuary</rdfs:label>
    </owl:NamedIndividual>
    


    <!-- http://purl.obolibrary.org/obo/GAZ_00253077 -->

    <owl:NamedIndividual rdf:about="http://purl.obolibrary.org/obo/GAZ_00253077">
        <obo:RO_0001025 rdf:resource="http://purl.obolibrary.org/obo/GAZ_00400058"/>
        <obo:IAO_0000115>A protected area. Established 1972.</obo:IAO_0000115>
        <oboInOwl:hasOBONamespace>GAZ</oboInOwl:hasOBONamespace>
        <oboInOwl:id>GAZ:00253077</oboInOwl:id>
        <rdfs:label>Taunsa Barrage Wildlife Sanctuary</rdfs:label>
    </owl:NamedIndividual>
    


    <!-- http://purl.obolibrary.org/obo/GAZ_00253078 -->

    <owl:NamedIndividual rdf:about="http://purl.obolibrary.org/obo/GAZ_00253078">
        <obo:RO_0001025 rdf:resource="http://purl.obolibrary.org/obo/GAZ_00080151"/>
        <obo:IAO_0000115>An abandoned water storage reservoir.</obo:IAO_0000115>
        <oboInOwl:hasOBONamespace>GAZ</oboInOwl:hasOBONamespace>
        <oboInOwl:id>GAZ:00253078</oboInOwl:id>
        <rdfs:label>Patisar Lake</rdfs:label>
    </owl:NamedIndividual>
    


    <!-- http://purl.obolibrary.org/obo/GAZ_00253080 -->

    <owl:NamedIndividual rdf:about="http://purl.obolibrary.org/obo/GAZ_00253080">
        <obo:RO_0001025 rdf:resource="http://purl.obolibrary.org/obo/GAZ_00248628"/>
        <obo:RO_0001025 rdf:resource="http://purl.obolibrary.org/obo/GAZ_00400092"/>
        <obo:IAO_0000115>A protected area. Protects 135 km of the Indus River from Sukkur Barrage upstream to the Guddu Barrage near Kashmor, Sind Province. Established 1974.</obo:IAO_0000115>
        <oboInOwl:hasOBONamespace>GAZ</oboInOwl:hasOBONamespace>
        <oboInOwl:id>GAZ:00253080</oboInOwl:id>
        <rdfs:label>Indus Dolphin Sanctuary</rdfs:label>
    </owl:NamedIndividual>
    


    <!-- http://purl.obolibrary.org/obo/GAZ_00253081 -->

    <owl:NamedIndividual rdf:about="http://purl.obolibrary.org/obo/GAZ_00253081">
        <rdf:type rdf:resource="http://purl.obolibrary.org/obo/ENVO_00000074"/>
        <obo:RO_0001025 rdf:resource="http://purl.obolibrary.org/obo/GAZ_00005251"/>
        <obo:RO_0001025 rdf:resource="http://purl.obolibrary.org/obo/GAZ_00248628"/>
        <obo:IAO_0000115>A barrage across the Indus river near the city of Sukkur, Pakistan. Constructed 1923-1932.</obo:IAO_0000115>
        <oboInOwl:hasOBONamespace>GAZ</oboInOwl:hasOBONamespace>
        <oboInOwl:id>GAZ:00253081</oboInOwl:id>
        <rdfs:label>Sukkur Barrage</rdfs:label>
    </owl:NamedIndividual>
    


    <!-- http://purl.obolibrary.org/obo/GAZ_00253082 -->

    <owl:NamedIndividual rdf:about="http://purl.obolibrary.org/obo/GAZ_00253082">
        <obo:RO_0001025 rdf:resource="http://purl.obolibrary.org/obo/GAZ_00005251"/>
        <obo:RO_0001025 rdf:resource="http://purl.obolibrary.org/obo/GAZ_00248628"/>
        <obo:IAO_0000115>A barrage across river Indus, near Sukkur in Pakistan. Constructed 1957-1962.</obo:IAO_0000115>
        <oboInOwl:hasOBONamespace>GAZ</oboInOwl:hasOBONamespace>
        <oboInOwl:id>GAZ:00253082</oboInOwl:id>
        <rdfs:label>Guddu Barrage</rdfs:label>
    </owl:NamedIndividual>
    


    <!-- http://purl.obolibrary.org/obo/GAZ_00253083 -->

    <owl:NamedIndividual rdf:about="http://purl.obolibrary.org/obo/GAZ_00253083">
        <obo:RO_0001025 rdf:resource="http://purl.obolibrary.org/obo/GAZ_00018545"/>
        <obo:IAO_0000115>A freshwater lake.</obo:IAO_0000115>
        <oboInOwl:hasOBONamespace>GAZ</oboInOwl:hasOBONamespace>
        <oboInOwl:id>GAZ:00253083</oboInOwl:id>
        <rdfs:label>Ghauspur Jheel</rdfs:label>
    </owl:NamedIndividual>
    


    <!-- http://purl.obolibrary.org/obo/GAZ_00253084 -->

    <owl:NamedIndividual rdf:about="http://purl.obolibrary.org/obo/GAZ_00253084">
        <obo:RO_0001025 rdf:resource="http://purl.obolibrary.org/obo/GAZ_00018545"/>
        <obo:IAO_0000115>A freshwater lake.</obo:IAO_0000115>
        <oboInOwl:hasOBONamespace>GAZ</oboInOwl:hasOBONamespace>
        <oboInOwl:id>GAZ:00253084</oboInOwl:id>
        <rdfs:label>Sindhi Dhoro Lake</rdfs:label>
    </owl:NamedIndividual>
    


    <!-- http://purl.obolibrary.org/obo/GAZ_00253085 -->

    <owl:NamedIndividual rdf:about="http://purl.obolibrary.org/obo/GAZ_00253085">
        <obo:RO_0001025 rdf:resource="http://purl.obolibrary.org/obo/GAZ_00400013"/>
        <obo:IAO_0000115>A Canal.</obo:IAO_0000115>
        <oboInOwl:hasOBONamespace>GAZ</oboInOwl:hasOBONamespace>
        <oboInOwl:id>GAZ:00253085</oboInOwl:id>
        <rdfs:label>Beroon Kirthar Canal</rdfs:label>
    </owl:NamedIndividual>
    


    <!-- http://purl.obolibrary.org/obo/GAZ_00253086 -->

    <owl:NamedIndividual rdf:about="http://purl.obolibrary.org/obo/GAZ_00253086">
        <obo:RO_0001025 rdf:resource="http://purl.obolibrary.org/obo/GAZ_00018553"/>
        <obo:IAO_0000115>A protected area. Includes a small, slightly brackish lake with extensive marshes on the floodplain of the Indus River; formerly an ancient arm of the Indus, but now about 30 km from the river. Established 1972-10.</obo:IAO_0000115>
        <oboInOwl:hasOBONamespace>GAZ</oboInOwl:hasOBONamespace>
        <oboInOwl:id>GAZ:00253086</oboInOwl:id>
        <rdfs:label>Drigh Lake Wildlife Sanctuary</rdfs:label>
    </owl:NamedIndividual>
    


    <!-- http://purl.obolibrary.org/obo/GAZ_00253087 -->

    <owl:NamedIndividual rdf:about="http://purl.obolibrary.org/obo/GAZ_00253087">
        <obo:RO_0001025 rdf:resource="http://purl.obolibrary.org/obo/GAZ_00018553"/>
        <obo:IAO_0000115>A lake. Located near Naseerabad, Larkana District, Sind Province.</obo:IAO_0000115>
        <oboInOwl:hasOBONamespace>GAZ</oboInOwl:hasOBONamespace>
        <oboInOwl:id>GAZ:00253087</oboInOwl:id>
        <rdfs:label>Hamal Katchri Lake</rdfs:label>
    </owl:NamedIndividual>
    


    <!-- http://purl.obolibrary.org/obo/GAZ_00253088 -->

    <owl:NamedIndividual rdf:about="http://purl.obolibrary.org/obo/GAZ_00253088">
        <obo:RO_0001025 rdf:resource="http://purl.obolibrary.org/obo/GAZ_00018553"/>
        <obo:IAO_0000115>A brackish lake. Located 10 km southeast of Dokri and 30 km SSW of Larkana. Larkana District, Sind Province.</obo:IAO_0000115>
        <oboInOwl:hasOBONamespace>GAZ</oboInOwl:hasOBONamespace>
        <oboInOwl:id>GAZ:00253088</oboInOwl:id>
        <rdfs:label>Pugri Lake</rdfs:label>
    </owl:NamedIndividual>
    


    <!-- http://purl.obolibrary.org/obo/GAZ_00253089 -->

    <owl:NamedIndividual rdf:about="http://purl.obolibrary.org/obo/GAZ_00253089">
        <obo:RO_0001025 rdf:resource="http://purl.obolibrary.org/obo/GAZ_00018552"/>
        <obo:IAO_0000115>A freshwater lake. Located west of Sehwan, 35 km SSW of Dadu, Dadu District, Sind Province.</obo:IAO_0000115>
        <oboInOwl:hasOBONamespace>GAZ</oboInOwl:hasOBONamespace>
        <oboInOwl:id>GAZ:00253089</oboInOwl:id>
        <rdfs:label>Manchar Lake</rdfs:label>
    </owl:NamedIndividual>
    


    <!-- http://purl.obolibrary.org/obo/GAZ_00253092 -->

    <owl:NamedIndividual rdf:about="http://purl.obolibrary.org/obo/GAZ_00253092">
        <obo:IAO_0000115>A saline lake.</obo:IAO_0000115>
        <oboInOwl:hasOBONamespace>GAZ</oboInOwl:hasOBONamespace>
        <oboInOwl:id>GAZ:00253092</oboInOwl:id>
        <rdfs:label>Soonhari Lake</rdfs:label>
    </owl:NamedIndividual>
    


    <!-- http://purl.obolibrary.org/obo/GAZ_00253093 -->

    <owl:NamedIndividual rdf:about="http://purl.obolibrary.org/obo/GAZ_00253093">
        <obo:IAO_0000115>A freshwater lake.</obo:IAO_0000115>
        <oboInOwl:hasOBONamespace>GAZ</oboInOwl:hasOBONamespace>
        <oboInOwl:id>GAZ:00253093</oboInOwl:id>
        <rdfs:label>Sadhori Lake</rdfs:label>
    </owl:NamedIndividual>
    


    <!-- http://purl.obolibrary.org/obo/GAZ_00253094 -->

    <owl:NamedIndividual rdf:about="http://purl.obolibrary.org/obo/GAZ_00253094">
        <obo:IAO_0000115>A brackish lake.</obo:IAO_0000115>
        <oboInOwl:hasOBONamespace>GAZ</oboInOwl:hasOBONamespace>
        <oboInOwl:id>GAZ:00253094</oboInOwl:id>
        <rdfs:label>Sanghriaro Lake</rdfs:label>
    </owl:NamedIndividual>
    


    <!-- http://purl.obolibrary.org/obo/GAZ_00253095 -->

    <owl:NamedIndividual rdf:about="http://purl.obolibrary.org/obo/GAZ_00253095">
        <obo:IAO_0000115>A lake.</obo:IAO_0000115>
        <oboInOwl:hasOBONamespace>GAZ</oboInOwl:hasOBONamespace>
        <oboInOwl:id>GAZ:00253095</oboInOwl:id>
        <rdfs:label>Baqar Lake</rdfs:label>
    </owl:NamedIndividual>
    


    <!-- http://purl.obolibrary.org/obo/GAZ_00253096 -->

    <owl:NamedIndividual rdf:about="http://purl.obolibrary.org/obo/GAZ_00253096">
        <obo:IAO_0000115>A lake.</obo:IAO_0000115>
        <oboInOwl:hasOBONamespace>GAZ</oboInOwl:hasOBONamespace>
        <oboInOwl:id>GAZ:00253096</oboInOwl:id>
        <rdfs:label>Purai Lake</rdfs:label>
    </owl:NamedIndividual>
    


    <!-- http://purl.obolibrary.org/obo/GAZ_00253097 -->

    <owl:NamedIndividual rdf:about="http://purl.obolibrary.org/obo/GAZ_00253097">
        <obo:IAO_0000115>A lake.</obo:IAO_0000115>
        <oboInOwl:hasOBONamespace>GAZ</oboInOwl:hasOBONamespace>
        <oboInOwl:id>GAZ:00253097</oboInOwl:id>
        <rdfs:label>Mitha Dhand</rdfs:label>
    </owl:NamedIndividual>
    


    <!-- http://purl.obolibrary.org/obo/GAZ_00253098 -->

    <owl:NamedIndividual rdf:about="http://purl.obolibrary.org/obo/GAZ_00253098">
        <obo:IAO_0000115>A lake.</obo:IAO_0000115>
        <oboInOwl:hasOBONamespace>GAZ</oboInOwl:hasOBONamespace>
        <oboInOwl:id>GAZ:00253098</oboInOwl:id>
        <rdfs:label>Rajpar Dhand</rdfs:label>
    </owl:NamedIndividual>
    


    <!-- http://purl.obolibrary.org/obo/GAZ_00253099 -->

    <owl:NamedIndividual rdf:about="http://purl.obolibrary.org/obo/GAZ_00253099">
        <obo:IAO_0000115>A lake.</obo:IAO_0000115>
        <oboInOwl:hasOBONamespace>GAZ</oboInOwl:hasOBONamespace>
        <oboInOwl:id>GAZ:00253099</oboInOwl:id>
        <rdfs:label>Dhanipat Lake</rdfs:label>
    </owl:NamedIndividual>
    


    <!-- http://purl.obolibrary.org/obo/GAZ_00253100 -->

    <owl:NamedIndividual rdf:about="http://purl.obolibrary.org/obo/GAZ_00253100">
        <obo:IAO_0000115>A lake.</obo:IAO_0000115>
        <oboInOwl:hasOBONamespace>GAZ</oboInOwl:hasOBONamespace>
        <oboInOwl:id>GAZ:00253100</oboInOwl:id>
        <rdfs:label>Keh-hari Lake</rdfs:label>
    </owl:NamedIndividual>
    


    <!-- http://purl.obolibrary.org/obo/GAZ_00253101 -->

    <owl:NamedIndividual rdf:about="http://purl.obolibrary.org/obo/GAZ_00253101">
        <obo:IAO_0000115>A lake.</obo:IAO_0000115>
        <oboInOwl:hasOBONamespace>GAZ</oboInOwl:hasOBONamespace>
        <oboInOwl:id>GAZ:00253101</oboInOwl:id>
        <rdfs:label>Jhal Dhand</rdfs:label>
    </owl:NamedIndividual>
    


    <!-- http://purl.obolibrary.org/obo/GAZ_00253102 -->

    <owl:NamedIndividual rdf:about="http://purl.obolibrary.org/obo/GAZ_00253102">
        <obo:IAO_0000115>A lake.</obo:IAO_0000115>
        <oboInOwl:hasOBONamespace>GAZ</oboInOwl:hasOBONamespace>
        <oboInOwl:id>GAZ:00253102</oboInOwl:id>
        <rdfs:label>Sainjoro Lake</rdfs:label>
    </owl:NamedIndividual>
    


    <!-- http://purl.obolibrary.org/obo/GAZ_00253103 -->

    <owl:NamedIndividual rdf:about="http://purl.obolibrary.org/obo/GAZ_00253103">
        <obo:IAO_0000115>A lake.</obo:IAO_0000115>
        <oboInOwl:hasOBONamespace>GAZ</oboInOwl:hasOBONamespace>
        <oboInOwl:id>GAZ:00253103</oboInOwl:id>
        <rdfs:label>Gajri Dhand</rdfs:label>
    </owl:NamedIndividual>
    


    <!-- http://purl.obolibrary.org/obo/GAZ_00253104 -->

    <owl:NamedIndividual rdf:about="http://purl.obolibrary.org/obo/GAZ_00253104">
        <obo:IAO_0000115>A lake.</obo:IAO_0000115>
        <oboInOwl:hasOBONamespace>GAZ</oboInOwl:hasOBONamespace>
        <oboInOwl:id>GAZ:00253104</oboInOwl:id>
        <rdfs:label>Simna Lake</rdfs:label>
    </owl:NamedIndividual>
    


    <!-- http://purl.obolibrary.org/obo/GAZ_00253105 -->

    <owl:NamedIndividual rdf:about="http://purl.obolibrary.org/obo/GAZ_00253105">
        <obo:IAO_0000115>A lake.</obo:IAO_0000115>
        <oboInOwl:hasOBONamespace>GAZ</oboInOwl:hasOBONamespace>
        <oboInOwl:id>GAZ:00253105</oboInOwl:id>
        <rdfs:label>Abad Dhand</rdfs:label>
    </owl:NamedIndividual>
    


    <!-- http://purl.obolibrary.org/obo/GAZ_00253106 -->

    <owl:NamedIndividual rdf:about="http://purl.obolibrary.org/obo/GAZ_00253106">
        <obo:IAO_0000115>A lake.</obo:IAO_0000115>
        <oboInOwl:hasOBONamespace>GAZ</oboInOwl:hasOBONamespace>
        <oboInOwl:id>GAZ:00253106</oboInOwl:id>
        <rdfs:label>Gujro Lake</rdfs:label>
    </owl:NamedIndividual>
    


    <!-- http://purl.obolibrary.org/obo/GAZ_00253107 -->

    <owl:NamedIndividual rdf:about="http://purl.obolibrary.org/obo/GAZ_00253107">
        <obo:IAO_0000115>A lake.</obo:IAO_0000115>
        <oboInOwl:hasOBONamespace>GAZ</oboInOwl:hasOBONamespace>
        <oboInOwl:id>GAZ:00253107</oboInOwl:id>
        <rdfs:label>Naro Lake</rdfs:label>
    </owl:NamedIndividual>
    


    <!-- http://purl.obolibrary.org/obo/GAZ_00253109 -->

    <owl:NamedIndividual rdf:about="http://purl.obolibrary.org/obo/GAZ_00253109">
        <obo:IAO_0000115>A lake.</obo:IAO_0000115>
        <oboInOwl:hasOBONamespace>GAZ</oboInOwl:hasOBONamespace>
        <oboInOwl:id>GAZ:00253109</oboInOwl:id>
        <rdfs:label>Wanahero Lake</rdfs:label>
    </owl:NamedIndividual>
    


    <!-- http://purl.obolibrary.org/obo/GAZ_00253110 -->

    <owl:NamedIndividual rdf:about="http://purl.obolibrary.org/obo/GAZ_00253110">
        <obo:IAO_0000115>A lake.</obo:IAO_0000115>
        <oboInOwl:hasOBONamespace>GAZ</oboInOwl:hasOBONamespace>
        <oboInOwl:id>GAZ:00253110</oboInOwl:id>
        <rdfs:label>Bothaar Lake</rdfs:label>
    </owl:NamedIndividual>
    


    <!-- http://purl.obolibrary.org/obo/GAZ_00253111 -->

    <owl:NamedIndividual rdf:about="http://purl.obolibrary.org/obo/GAZ_00253111">
        <obo:IAO_0000115>A lake.</obo:IAO_0000115>
        <oboInOwl:hasOBONamespace>GAZ</oboInOwl:hasOBONamespace>
        <oboInOwl:id>GAZ:00253111</oboInOwl:id>
        <rdfs:label>Wingio Lake</rdfs:label>
    </owl:NamedIndividual>
    


    <!-- http://purl.obolibrary.org/obo/GAZ_00253112 -->

    <owl:NamedIndividual rdf:about="http://purl.obolibrary.org/obo/GAZ_00253112">
        <obo:IAO_0000115>A lake.</obo:IAO_0000115>
        <oboInOwl:hasOBONamespace>GAZ</oboInOwl:hasOBONamespace>
        <oboInOwl:id>GAZ:00253112</oboInOwl:id>
        <rdfs:label>Gujri Lake</rdfs:label>
    </owl:NamedIndividual>
    


    <!-- http://purl.obolibrary.org/obo/GAZ_00253113 -->

    <owl:NamedIndividual rdf:about="http://purl.obolibrary.org/obo/GAZ_00253113">
        <obo:IAO_0000115>A lake.</obo:IAO_0000115>
        <oboInOwl:hasOBONamespace>GAZ</oboInOwl:hasOBONamespace>
        <oboInOwl:id>GAZ:00253113</oboInOwl:id>
        <rdfs:label>Kinri Lake</rdfs:label>
    </owl:NamedIndividual>
    


    <!-- http://purl.obolibrary.org/obo/GAZ_00253114 -->

    <owl:NamedIndividual rdf:about="http://purl.obolibrary.org/obo/GAZ_00253114">
        <obo:IAO_0000115>A lake.</obo:IAO_0000115>
        <oboInOwl:hasOBONamespace>GAZ</oboInOwl:hasOBONamespace>
        <oboInOwl:id>GAZ:00253114</oboInOwl:id>
        <rdfs:label>Palaro Lake</rdfs:label>
    </owl:NamedIndividual>
    


    <!-- http://purl.obolibrary.org/obo/GAZ_00253115 -->

    <owl:NamedIndividual rdf:about="http://purl.obolibrary.org/obo/GAZ_00253115">
        <obo:IAO_0000115>A lake.</obo:IAO_0000115>
        <oboInOwl:hasOBONamespace>GAZ</oboInOwl:hasOBONamespace>
        <oboInOwl:id>GAZ:00253115</oboInOwl:id>
        <rdfs:label>Kalanger Lake</rdfs:label>
    </owl:NamedIndividual>
    


    <!-- http://purl.obolibrary.org/obo/GAZ_00253116 -->

    <owl:NamedIndividual rdf:about="http://purl.obolibrary.org/obo/GAZ_00253116">
        <obo:IAO_0000115>A lake.</obo:IAO_0000115>
        <oboInOwl:hasOBONamespace>GAZ</oboInOwl:hasOBONamespace>
        <oboInOwl:id>GAZ:00253116</oboInOwl:id>
        <rdfs:label>Rarr Lake</rdfs:label>
    </owl:NamedIndividual>
    


    <!-- http://purl.obolibrary.org/obo/GAZ_00253117 -->

    <owl:NamedIndividual rdf:about="http://purl.obolibrary.org/obo/GAZ_00253117">
        <obo:IAO_0000115>A lake.</obo:IAO_0000115>
        <oboInOwl:hasOBONamespace>GAZ</oboInOwl:hasOBONamespace>
        <oboInOwl:id>GAZ:00253117</oboInOwl:id>
        <rdfs:label>Ithpar Lake</rdfs:label>
    </owl:NamedIndividual>
    


    <!-- http://purl.obolibrary.org/obo/GAZ_00253118 -->

    <owl:NamedIndividual rdf:about="http://purl.obolibrary.org/obo/GAZ_00253118">
        <obo:IAO_0000115>A lake.</obo:IAO_0000115>
        <oboInOwl:hasOBONamespace>GAZ</oboInOwl:hasOBONamespace>
        <oboInOwl:id>GAZ:00253118</oboInOwl:id>
        <rdfs:label>Dino Jakhro Ji Dhand</rdfs:label>
    </owl:NamedIndividual>
    


    <!-- http://purl.obolibrary.org/obo/GAZ_00253119 -->

    <owl:NamedIndividual rdf:about="http://purl.obolibrary.org/obo/GAZ_00253119">
        <obo:IAO_0000115>A lake.</obo:IAO_0000115>
        <oboInOwl:hasOBONamespace>GAZ</oboInOwl:hasOBONamespace>
        <oboInOwl:id>GAZ:00253119</oboInOwl:id>
        <rdfs:label>Mehmood Wan Dhand</rdfs:label>
    </owl:NamedIndividual>
    


    <!-- http://purl.obolibrary.org/obo/GAZ_00253120 -->

    <owl:NamedIndividual rdf:about="http://purl.obolibrary.org/obo/GAZ_00253120">
        <obo:IAO_0000115>A lake.</obo:IAO_0000115>
        <oboInOwl:hasOBONamespace>GAZ</oboInOwl:hasOBONamespace>
        <oboInOwl:id>GAZ:00253120</oboInOwl:id>
        <rdfs:label>Burthi Lake</rdfs:label>
    </owl:NamedIndividual>
    


    <!-- http://purl.obolibrary.org/obo/GAZ_00253121 -->

    <owl:NamedIndividual rdf:about="http://purl.obolibrary.org/obo/GAZ_00253121">
        <obo:IAO_0000115>A lake.</obo:IAO_0000115>
        <oboInOwl:hasOBONamespace>GAZ</oboInOwl:hasOBONamespace>
        <oboInOwl:id>GAZ:00253121</oboInOwl:id>
        <rdfs:label>Loonhar Lake</rdfs:label>
    </owl:NamedIndividual>
    


    <!-- http://purl.obolibrary.org/obo/GAZ_00253122 -->

    <owl:NamedIndividual rdf:about="http://purl.obolibrary.org/obo/GAZ_00253122">
        <obo:IAO_0000115>A lake.</obo:IAO_0000115>
        <oboInOwl:hasOBONamespace>GAZ</oboInOwl:hasOBONamespace>
        <oboInOwl:id>GAZ:00253122</oboInOwl:id>
        <rdfs:label>Dabri Lake</rdfs:label>
    </owl:NamedIndividual>
    


    <!-- http://purl.obolibrary.org/obo/GAZ_00253123 -->

    <owl:NamedIndividual rdf:about="http://purl.obolibrary.org/obo/GAZ_00253123">
        <obo:RO_0001025 rdf:resource="http://purl.obolibrary.org/obo/GAZ_00400085"/>
        <obo:IAO_0000115>A group of eleven shallow, fresh or slightly brackish lakes and associated marshes on the eastern edge of the Indus plain near the town of Tando Bago.</obo:IAO_0000115>
        <oboInOwl:hasOBONamespace>GAZ</oboInOwl:hasOBONamespace>
        <oboInOwl:id>GAZ:00253123</oboInOwl:id>
        <rdfs:label>Tando Bago Lakes</rdfs:label>
    </owl:NamedIndividual>
    


    <!-- http://purl.obolibrary.org/obo/GAZ_00253124 -->

    <owl:NamedIndividual rdf:about="http://purl.obolibrary.org/obo/GAZ_00253124">
        <obo:RO_0001025 rdf:resource="http://purl.obolibrary.org/obo/GAZ_00253123"/>
        <obo:IAO_0000115>A brackish lake.</obo:IAO_0000115>
        <oboInOwl:hasOBONamespace>GAZ</oboInOwl:hasOBONamespace>
        <oboInOwl:id>GAZ:00253124</oboInOwl:id>
        <rdfs:label>Phoosna I Lake</rdfs:label>
    </owl:NamedIndividual>
    


    <!-- http://purl.obolibrary.org/obo/GAZ_00253125 -->

    <owl:NamedIndividual rdf:about="http://purl.obolibrary.org/obo/GAZ_00253125">
        <obo:RO_0001025 rdf:resource="http://purl.obolibrary.org/obo/GAZ_00253123"/>
        <obo:IAO_0000115>A brackish lake.</obo:IAO_0000115>
        <oboInOwl:hasOBONamespace>GAZ</oboInOwl:hasOBONamespace>
        <oboInOwl:id>GAZ:00253125</oboInOwl:id>
        <rdfs:label>Phoosna II Lake</rdfs:label>
    </owl:NamedIndividual>
    


    <!-- http://purl.obolibrary.org/obo/GAZ_00253126 -->

    <owl:NamedIndividual rdf:about="http://purl.obolibrary.org/obo/GAZ_00253126">
        <obo:RO_0001025 rdf:resource="http://purl.obolibrary.org/obo/GAZ_00253123"/>
        <obo:IAO_0000115>A freshwater lake.</obo:IAO_0000115>
        <oboInOwl:hasOBONamespace>GAZ</oboInOwl:hasOBONamespace>
        <oboInOwl:id>GAZ:00253126</oboInOwl:id>
        <rdfs:label>Charwo Lake</rdfs:label>
    </owl:NamedIndividual>
    


    <!-- http://purl.obolibrary.org/obo/GAZ_00253127 -->

    <owl:NamedIndividual rdf:about="http://purl.obolibrary.org/obo/GAZ_00253127">
        <obo:RO_0001025 rdf:resource="http://purl.obolibrary.org/obo/GAZ_00253123"/>
        <obo:IAO_0000115>A freshwater lake.</obo:IAO_0000115>
        <oboInOwl:hasOBONamespace>GAZ</oboInOwl:hasOBONamespace>
        <oboInOwl:id>GAZ:00253127</oboInOwl:id>
        <rdfs:label>Khanjo Lake</rdfs:label>
    </owl:NamedIndividual>
    


    <!-- http://purl.obolibrary.org/obo/GAZ_00253128 -->

    <owl:NamedIndividual rdf:about="http://purl.obolibrary.org/obo/GAZ_00253128">
        <obo:RO_0001025 rdf:resource="http://purl.obolibrary.org/obo/GAZ_00253123"/>
        <oboInOwl:hasOBONamespace>GAZ</oboInOwl:hasOBONamespace>
        <oboInOwl:id>GAZ:00253128</oboInOwl:id>
        <rdfs:label>Jan Lake</rdfs:label>
    </owl:NamedIndividual>
    


    <!-- http://purl.obolibrary.org/obo/GAZ_00253129 -->

    <owl:NamedIndividual rdf:about="http://purl.obolibrary.org/obo/GAZ_00253129">
        <obo:RO_0001025 rdf:resource="http://purl.obolibrary.org/obo/GAZ_00253123"/>
        <oboInOwl:hasOBONamespace>GAZ</oboInOwl:hasOBONamespace>
        <oboInOwl:id>GAZ:00253129</oboInOwl:id>
        <rdfs:label>Jaffarali Lake</rdfs:label>
    </owl:NamedIndividual>
    


    <!-- http://purl.obolibrary.org/obo/GAZ_00253130 -->

    <owl:NamedIndividual rdf:about="http://purl.obolibrary.org/obo/GAZ_00253130">
        <obo:RO_0001025 rdf:resource="http://purl.obolibrary.org/obo/GAZ_00253123"/>
        <oboInOwl:hasOBONamespace>GAZ</oboInOwl:hasOBONamespace>
        <oboInOwl:id>GAZ:00253130</oboInOwl:id>
        <rdfs:label>Nira Dhand</rdfs:label>
    </owl:NamedIndividual>
    


    <!-- http://purl.obolibrary.org/obo/GAZ_00253131 -->

    <owl:NamedIndividual rdf:about="http://purl.obolibrary.org/obo/GAZ_00253131">
        <obo:RO_0001025 rdf:resource="http://purl.obolibrary.org/obo/GAZ_00253123"/>
        <oboInOwl:hasOBONamespace>GAZ</oboInOwl:hasOBONamespace>
        <oboInOwl:id>GAZ:00253131</oboInOwl:id>
        <rdfs:label>Maachori Dhand</rdfs:label>
    </owl:NamedIndividual>
    


    <!-- http://purl.obolibrary.org/obo/GAZ_00253132 -->

    <owl:NamedIndividual rdf:about="http://purl.obolibrary.org/obo/GAZ_00253132">
        <obo:RO_0001025 rdf:resource="http://purl.obolibrary.org/obo/GAZ_00253123"/>
        <obo:IAO_0000115>A lake.</obo:IAO_0000115>
        <oboInOwl:hasOBONamespace>GAZ</oboInOwl:hasOBONamespace>
        <oboInOwl:id>GAZ:00253132</oboInOwl:id>
        <rdfs:label>Dabhka Lake</rdfs:label>
    </owl:NamedIndividual>
    


    <!-- http://purl.obolibrary.org/obo/GAZ_00253133 -->

    <owl:NamedIndividual rdf:about="http://purl.obolibrary.org/obo/GAZ_00253133">
        <obo:RO_0001025 rdf:resource="http://purl.obolibrary.org/obo/GAZ_00253123"/>
        <obo:IAO_0000115>A lake.</obo:IAO_0000115>
        <oboInOwl:hasOBONamespace>GAZ</oboInOwl:hasOBONamespace>
        <oboInOwl:id>GAZ:00253133</oboInOwl:id>
        <rdfs:label>Soonar Lake</rdfs:label>
    </owl:NamedIndividual>
    


    <!-- http://purl.obolibrary.org/obo/GAZ_00253134 -->

    <owl:NamedIndividual rdf:about="http://purl.obolibrary.org/obo/GAZ_00253134">
        <obo:RO_0001025 rdf:resource="http://purl.obolibrary.org/obo/GAZ_00253123"/>
        <obo:IAO_0000115>A lake.</obo:IAO_0000115>
        <oboInOwl:hasOBONamespace>GAZ</oboInOwl:hasOBONamespace>
        <oboInOwl:id>GAZ:00253134</oboInOwl:id>
        <rdfs:label>Sumro Lake</rdfs:label>
    </owl:NamedIndividual>
    


    <!-- http://purl.obolibrary.org/obo/GAZ_00253135 -->

    <owl:NamedIndividual rdf:about="http://purl.obolibrary.org/obo/GAZ_00253135">
        <obo:RO_0001025 rdf:resource="http://purl.obolibrary.org/obo/GAZ_00400085"/>
        <obo:IAO_0000115>A large area of very shallow brackish lagoons and wet mudflats at the end of drainage canals in the eastern part of the Indus delta, on the edge of the salt flats of the Great Rann of Kutch.</obo:IAO_0000115>
        <oboInOwl:hasOBONamespace>GAZ</oboInOwl:hasOBONamespace>
        <oboInOwl:id>GAZ:00253135</oboInOwl:id>
        <rdfs:label>Badin and Kadhan Lagoons</rdfs:label>
    </owl:NamedIndividual>
    


    <!-- http://purl.obolibrary.org/obo/GAZ_00253136 -->

    <owl:NamedIndividual rdf:about="http://purl.obolibrary.org/obo/GAZ_00253136">
        <obo:RO_0001025 rdf:resource="http://purl.obolibrary.org/obo/GAZ_00253135"/>
        <obo:IAO_0000115>A lagoon.</obo:IAO_0000115>
        <oboInOwl:hasOBONamespace>GAZ</oboInOwl:hasOBONamespace>
        <oboInOwl:id>GAZ:00253136</oboInOwl:id>
        <rdfs:label>Warharo Lake</rdfs:label>
    </owl:NamedIndividual>
    


    <!-- http://purl.obolibrary.org/obo/GAZ_00253137 -->

    <owl:NamedIndividual rdf:about="http://purl.obolibrary.org/obo/GAZ_00253137">
        <obo:RO_0001025 rdf:resource="http://purl.obolibrary.org/obo/GAZ_00253135"/>
        <obo:IAO_0000115>A lagoon. Located at the end of the Kara Gungro Outfall Drain near Golarchi.</obo:IAO_0000115>
        <oboInOwl:hasOBONamespace>GAZ</oboInOwl:hasOBONamespace>
        <oboInOwl:id>GAZ:00253137</oboInOwl:id>
        <rdfs:label>Kur Lagoon</rdfs:label>
    </owl:NamedIndividual>
    


    <!-- http://purl.obolibrary.org/obo/GAZ_00253138 -->

    <owl:NamedIndividual rdf:about="http://purl.obolibrary.org/obo/GAZ_00253138">
        <obo:RO_0001025 rdf:resource="http://purl.obolibrary.org/obo/GAZ_00253135"/>
        <obo:IAO_0000115>A lagoon.</obo:IAO_0000115>
        <oboInOwl:hasOBONamespace>GAZ</oboInOwl:hasOBONamespace>
        <oboInOwl:id>GAZ:00253138</oboInOwl:id>
        <rdfs:label>Dahee Lake</rdfs:label>
    </owl:NamedIndividual>
    


    <!-- http://purl.obolibrary.org/obo/GAZ_00253139 -->

    <owl:NamedIndividual rdf:about="http://purl.obolibrary.org/obo/GAZ_00253139">
        <obo:RO_0001025 rdf:resource="http://purl.obolibrary.org/obo/GAZ_00253135"/>
        <obo:IAO_0000115>A lagoon.</obo:IAO_0000115>
        <oboInOwl:hasOBONamespace>GAZ</oboInOwl:hasOBONamespace>
        <oboInOwl:id>GAZ:00253139</oboInOwl:id>
        <rdfs:label>Matchary Dhand</rdfs:label>
    </owl:NamedIndividual>
    


    <!-- http://purl.obolibrary.org/obo/GAZ_00253140 -->

    <owl:NamedIndividual rdf:about="http://purl.obolibrary.org/obo/GAZ_00253140">
        <obo:RO_0001025 rdf:resource="http://purl.obolibrary.org/obo/GAZ_00253135"/>
        <obo:IAO_0000115>A lagoon.</obo:IAO_0000115>
        <oboInOwl:hasOBONamespace>GAZ</oboInOwl:hasOBONamespace>
        <oboInOwl:id>GAZ:00253140</oboInOwl:id>
        <rdfs:label>Nurr-ri</rdfs:label>
    </owl:NamedIndividual>
    


    <!-- http://purl.obolibrary.org/obo/GAZ_00253141 -->

    <owl:NamedIndividual rdf:about="http://purl.obolibrary.org/obo/GAZ_00253141">
        <obo:RO_0001025 rdf:resource="http://purl.obolibrary.org/obo/GAZ_00253135"/>
        <obo:IAO_0000115>A lagoon.</obo:IAO_0000115>
        <oboInOwl:hasOBONamespace>GAZ</oboInOwl:hasOBONamespace>
        <oboInOwl:id>GAZ:00253141</oboInOwl:id>
        <rdfs:label>Loonarh Lake</rdfs:label>
    </owl:NamedIndividual>
    


    <!-- http://purl.obolibrary.org/obo/GAZ_00253142 -->

    <owl:NamedIndividual rdf:about="http://purl.obolibrary.org/obo/GAZ_00253142">
        <obo:RO_0001025 rdf:resource="http://purl.obolibrary.org/obo/GAZ_00253135"/>
        <obo:IAO_0000115>A lagoon.</obo:IAO_0000115>
        <oboInOwl:hasOBONamespace>GAZ</oboInOwl:hasOBONamespace>
        <oboInOwl:id>GAZ:00253142</oboInOwl:id>
        <rdfs:label>Sandhoo Lake</rdfs:label>
    </owl:NamedIndividual>
    


    <!-- http://purl.obolibrary.org/obo/GAZ_00253143 -->

    <owl:NamedIndividual rdf:about="http://purl.obolibrary.org/obo/GAZ_00253143">
        <obo:RO_0001025 rdf:resource="http://purl.obolibrary.org/obo/GAZ_00253135"/>
        <obo:IAO_0000115>A lagoon.</obo:IAO_0000115>
        <oboInOwl:hasOBONamespace>GAZ</oboInOwl:hasOBONamespace>
        <oboInOwl:id>GAZ:00253143</oboInOwl:id>
        <rdfs:label>Shaikh Kerio Peer</rdfs:label>
    </owl:NamedIndividual>
    


    <!-- http://purl.obolibrary.org/obo/GAZ_00253144 -->

    <owl:NamedIndividual rdf:about="http://purl.obolibrary.org/obo/GAZ_00253144">
        <obo:RO_0001025 rdf:resource="http://purl.obolibrary.org/obo/GAZ_00400091"/>
        <obo:IAO_0000115>A brackish/saline lake.</obo:IAO_0000115>
        <oboInOwl:hasOBONamespace>GAZ</oboInOwl:hasOBONamespace>
        <oboInOwl:id>GAZ:00253144</oboInOwl:id>
        <rdfs:label>Jafri Lake</rdfs:label>
    </owl:NamedIndividual>
    


    <!-- http://purl.obolibrary.org/obo/GAZ_00253145 -->

    <owl:NamedIndividual rdf:about="http://purl.obolibrary.org/obo/GAZ_00253145">
        <obo:RO_0001025 rdf:resource="http://purl.obolibrary.org/obo/GAZ_00400091"/>
        <obo:IAO_0000115>A large salt waste extending east from the region of Shahbunder for about 35 km, Thatta District, Sind Province.</obo:IAO_0000115>
        <oboInOwl:hasOBONamespace>GAZ</oboInOwl:hasOBONamespace>
        <oboInOwl:id>GAZ:00253145</oboInOwl:id>
        <rdfs:label>Shahbunder Salt Waste</rdfs:label>
    </owl:NamedIndividual>
    


    <!-- http://purl.obolibrary.org/obo/GAZ_00253146 -->

    <owl:NamedIndividual rdf:about="http://purl.obolibrary.org/obo/GAZ_00253146">
        <obo:RO_0001025 rdf:resource="http://purl.obolibrary.org/obo/GAZ_00400091"/>
        <obo:IAO_0000115>A Taluka in Thatta District, Sindh.</obo:IAO_0000115>
        <oboInOwl:hasOBONamespace>GAZ</oboInOwl:hasOBONamespace>
        <oboInOwl:id>GAZ:00253146</oboInOwl:id>
        <rdfs:label>Kharo Chan Taluka</rdfs:label>
    </owl:NamedIndividual>
    


    <!-- http://purl.obolibrary.org/obo/GAZ_00253147 -->

    <owl:NamedIndividual rdf:about="http://purl.obolibrary.org/obo/GAZ_00253147">
        <obo:RO_0001025 rdf:resource="http://purl.obolibrary.org/obo/GAZ_00400091"/>
        <obo:IAO_0000115>A Taluka in Thatta District, Sindh.</obo:IAO_0000115>
        <oboInOwl:hasOBONamespace>GAZ</oboInOwl:hasOBONamespace>
        <oboInOwl:id>GAZ:00253147</oboInOwl:id>
        <rdfs:label>Keti Bander Taluka</rdfs:label>
    </owl:NamedIndividual>
    


    <!-- http://purl.obolibrary.org/obo/GAZ_00253148 -->

    <owl:NamedIndividual rdf:about="http://purl.obolibrary.org/obo/GAZ_00253148">
        <obo:RO_0001025 rdf:resource="http://purl.obolibrary.org/obo/GAZ_00400091"/>
        <obo:IAO_0000115>A fresh to brackish lake. Located 10 km SSW of Sujawal, Sind Province.</obo:IAO_0000115>
        <oboInOwl:hasOBONamespace>GAZ</oboInOwl:hasOBONamespace>
        <oboInOwl:id>GAZ:00253148</oboInOwl:id>
        <rdfs:label>Mahboob Shah Lake</rdfs:label>
    </owl:NamedIndividual>
    


    <!-- http://purl.obolibrary.org/obo/GAZ_00253151 -->

    <owl:NamedIndividual rdf:about="http://purl.obolibrary.org/obo/GAZ_00253151">
        <obo:RO_0001025 rdf:resource="http://purl.obolibrary.org/obo/GAZ_00400091"/>
        <obo:IAO_0000115>A protected area. Established 1977.</obo:IAO_0000115>
        <oboInOwl:hasOBONamespace>GAZ</oboInOwl:hasOBONamespace>
        <oboInOwl:id>GAZ:00253151</oboInOwl:id>
        <rdfs:label>Hadero Lake Wildlife Sanctuary</rdfs:label>
    </owl:NamedIndividual>
    


    <!-- http://purl.obolibrary.org/obo/GAZ_00253152 -->

    <owl:NamedIndividual rdf:about="http://purl.obolibrary.org/obo/GAZ_00253152">
        <obo:RO_0001025 rdf:resource="http://purl.obolibrary.org/obo/GAZ_00400091"/>
        <obo:IAO_0000115>A protected area. Established 1977.</obo:IAO_0000115>
        <oboInOwl:hasOBONamespace>GAZ</oboInOwl:hasOBONamespace>
        <oboInOwl:id>GAZ:00253152</oboInOwl:id>
        <rdfs:label>Haleji Lake Wildlife Sanctuary</rdfs:label>
    </owl:NamedIndividual>
    


    <!-- http://purl.obolibrary.org/obo/GAZ_00253153 -->

    <owl:NamedIndividual rdf:about="http://purl.obolibrary.org/obo/GAZ_00253153">
        <obo:RO_0001025 rdf:resource="http://purl.obolibrary.org/obo/GAZ_00253152"/>
        <obo:IAO_0000115>A freshwater lake. It can be filled from Haleji Lake via a by-pass regulator.</obo:IAO_0000115>
        <oboInOwl:hasOBONamespace>GAZ</oboInOwl:hasOBONamespace>
        <oboInOwl:id>GAZ:00253153</oboInOwl:id>
        <rdfs:label>Chateji Dhand</rdfs:label>
    </owl:NamedIndividual>
    


    <!-- http://purl.obolibrary.org/obo/GAZ_00253154 -->

    <owl:NamedIndividual rdf:about="http://purl.obolibrary.org/obo/GAZ_00253154">
        <obo:RO_0001025 rdf:resource="http://purl.obolibrary.org/obo/GAZ_00009471"/>
        <obo:IAO_0000115>A protected area. Established 1972.</obo:IAO_0000115>
        <oboInOwl:hasOBONamespace>GAZ</oboInOwl:hasOBONamespace>
        <oboInOwl:id>GAZ:00253154</oboInOwl:id>
        <rdfs:label>Hub Dam Wildlife Sanctuary</rdfs:label>
    </owl:NamedIndividual>
    


    <!-- http://purl.obolibrary.org/obo/GAZ_00253155 -->

    <owl:NamedIndividual rdf:about="http://purl.obolibrary.org/obo/GAZ_00253155">
        <obo:RO_0001025 rdf:resource="http://purl.obolibrary.org/obo/GAZ_00009471"/>
        <obo:IAO_0000115>A bay. Located on the coast southwest of Karachi City, Sind Province.</obo:IAO_0000115>
        <oboInOwl:hasOBONamespace>GAZ</oboInOwl:hasOBONamespace>
        <oboInOwl:id>GAZ:00253155</oboInOwl:id>
        <rdfs:label>Hawkes Bay</rdfs:label>
    </owl:NamedIndividual>
    


    <!-- http://purl.obolibrary.org/obo/GAZ_00253156 -->

    <owl:NamedIndividual rdf:about="http://purl.obolibrary.org/obo/GAZ_00253156">
        <obo:RO_0001025 rdf:resource="http://purl.obolibrary.org/obo/GAZ_00005248"/>
        <obo:IAO_0000115>A bay.</obo:IAO_0000115>
        <oboInOwl:hasOBONamespace>GAZ</oboInOwl:hasOBONamespace>
        <oboInOwl:id>GAZ:00253156</oboInOwl:id>
        <rdfs:label>Sonmiani Bay</rdfs:label>
    </owl:NamedIndividual>
    


    <!-- http://purl.obolibrary.org/obo/GAZ_00253157 -->

    <owl:NamedIndividual rdf:about="http://purl.obolibrary.org/obo/GAZ_00253157">
        <obo:RO_0001025 rdf:resource="http://purl.obolibrary.org/obo/GAZ_00400020"/>
        <obo:IAO_0000115>A lagoon.</obo:IAO_0000115>
        <oboInOwl:hasOBONamespace>GAZ</oboInOwl:hasOBONamespace>
        <oboInOwl:id>GAZ:00253157</oboInOwl:id>
        <rdfs:label>Miani Hor</rdfs:label>
    </owl:NamedIndividual>
    


    <!-- http://purl.obolibrary.org/obo/GAZ_00253158 -->

    <owl:NamedIndividual rdf:about="http://purl.obolibrary.org/obo/GAZ_00253158">
        <obo:RO_0001025 rdf:resource="http://purl.obolibrary.org/obo/GAZ_00009471"/>
        <obo:IAO_0000115>A protected area.</obo:IAO_0000115>
        <oboInOwl:hasOBONamespace>GAZ</oboInOwl:hasOBONamespace>
        <oboInOwl:id>GAZ:00253158</oboInOwl:id>
        <rdfs:label>Hawkes Bay/Sandspit Wildlife Sanctuary</rdfs:label>
    </owl:NamedIndividual>
    


    <!-- http://purl.obolibrary.org/obo/GAZ_00253159 -->

    <owl:NamedIndividual rdf:about="http://purl.obolibrary.org/obo/GAZ_00253159">
        <obo:RO_0001025 rdf:resource="http://purl.obolibrary.org/obo/GAZ_00007411"/>
        <obo:IAO_0000115>A port. It is located between the towns of Kiamari and Saddar, close to the heart of old Karachi.</obo:IAO_0000115>
        <oboInOwl:hasOBONamespace>GAZ</oboInOwl:hasOBONamespace>
        <oboInOwl:id>GAZ:00253159</oboInOwl:id>
        <rdfs:label>Port of Karachi</rdfs:label>
    </owl:NamedIndividual>
    


    <!-- http://purl.obolibrary.org/obo/GAZ_00253160 -->

    <owl:NamedIndividual rdf:about="http://purl.obolibrary.org/obo/GAZ_00253160">
        <obo:RO_0001025 rdf:resource="http://purl.obolibrary.org/obo/GAZ_00005251"/>
        <obo:IAO_0000115>The delta of the Indus River. A Ramsar Site.</obo:IAO_0000115>
        <oboInOwl:hasOBONamespace>GAZ</oboInOwl:hasOBONamespace>
        <oboInOwl:id>GAZ:00253160</oboInOwl:id>
        <rdfs:label>Indus River Delta</rdfs:label>
    </owl:NamedIndividual>
    


    <!-- http://purl.obolibrary.org/obo/GAZ_00253161 -->

    <owl:NamedIndividual rdf:about="http://purl.obolibrary.org/obo/GAZ_00253161">
        <obo:RO_0001025 rdf:resource="http://purl.obolibrary.org/obo/GAZ_00253160"/>
        <obo:IAO_0000115>A tidal creek.</obo:IAO_0000115>
        <oboInOwl:hasOBONamespace>GAZ</oboInOwl:hasOBONamespace>
        <oboInOwl:id>GAZ:00253161</oboInOwl:id>
        <rdfs:label>Korangi Creek</rdfs:label>
    </owl:NamedIndividual>
    


    <!-- http://purl.obolibrary.org/obo/GAZ_00253162 -->

    <owl:NamedIndividual rdf:about="http://purl.obolibrary.org/obo/GAZ_00253162">
        <obo:RO_0001025 rdf:resource="http://purl.obolibrary.org/obo/GAZ_00253160"/>
        <obo:IAO_0000115>A tidal creek.</obo:IAO_0000115>
        <oboInOwl:hasOBONamespace>GAZ</oboInOwl:hasOBONamespace>
        <oboInOwl:id>GAZ:00253162</oboInOwl:id>
        <rdfs:label>Gharo Creek</rdfs:label>
    </owl:NamedIndividual>
    


    <!-- http://purl.obolibrary.org/obo/GAZ_00253163 -->

    <owl:NamedIndividual rdf:about="http://purl.obolibrary.org/obo/GAZ_00253163">
        <obo:RO_0001025 rdf:resource="http://purl.obolibrary.org/obo/GAZ_00400091"/>
        <obo:IAO_0000115>A protected area. Established 1975.</obo:IAO_0000115>
        <oboInOwl:hasOBONamespace>GAZ</oboInOwl:hasOBONamespace>
        <oboInOwl:id>GAZ:00253163</oboInOwl:id>
        <rdfs:label>Kalri Lake Wildlife Sanctuary</rdfs:label>
    </owl:NamedIndividual>
    


    <!-- http://purl.obolibrary.org/obo/GAZ_00253164 -->

    <owl:NamedIndividual rdf:about="http://purl.obolibrary.org/obo/GAZ_00253164">
        <obo:RO_0001025 rdf:resource="http://purl.obolibrary.org/obo/GAZ_00253160"/>
        <obo:IAO_0000115>A protected area. Established 1977.</obo:IAO_0000115>
        <oboInOwl:hasOBONamespace>GAZ</oboInOwl:hasOBONamespace>
        <oboInOwl:id>GAZ:00253164</oboInOwl:id>
        <rdfs:label>Keti Bundar North Wildlife Sanctuary</rdfs:label>
    </owl:NamedIndividual>
    


    <!-- http://purl.obolibrary.org/obo/GAZ_00253165 -->

    <owl:NamedIndividual rdf:about="http://purl.obolibrary.org/obo/GAZ_00253165">
        <obo:RO_0001025 rdf:resource="http://purl.obolibrary.org/obo/GAZ_00253160"/>
        <obo:IAO_0000115>A protected area. Established 1977.</obo:IAO_0000115>
        <oboInOwl:hasOBONamespace>GAZ</oboInOwl:hasOBONamespace>
        <oboInOwl:id>GAZ:00253165</oboInOwl:id>
        <rdfs:label>Keti Bundar South Wildlife Sanctuary</rdfs:label>
    </owl:NamedIndividual>
    


    <!-- http://purl.obolibrary.org/obo/GAZ_00253166 -->

    <owl:NamedIndividual rdf:about="http://purl.obolibrary.org/obo/GAZ_00253166">
        <obo:RO_0001025 rdf:resource="http://purl.obolibrary.org/obo/GAZ_00400009"/>
        <obo:IAO_0000115>A protected area. Established 1983.</obo:IAO_0000115>
        <oboInOwl:hasOBONamespace>GAZ</oboInOwl:hasOBONamespace>
        <oboInOwl:id>GAZ:00253166</oboInOwl:id>
        <rdfs:label>Bund Khushdil Khan Game Reserve</rdfs:label>
    </owl:NamedIndividual>
    


    <!-- http://purl.obolibrary.org/obo/GAZ_00253167 -->

    <owl:NamedIndividual rdf:about="http://purl.obolibrary.org/obo/GAZ_00253167">
        <obo:RO_0001025 rdf:resource="http://purl.obolibrary.org/obo/GAZ_00253166"/>
        <obo:IAO_0000115>A water storage reservoir. Located 50 km NNW of Quetta, Pishin District, Baluchistan Province.</obo:IAO_0000115>
        <oboInOwl:hasOBONamespace>GAZ</oboInOwl:hasOBONamespace>
        <oboInOwl:id>GAZ:00253167</oboInOwl:id>
        <rdfs:label>Bund Khushdil Khan</rdfs:label>
    </owl:NamedIndividual>
    


    <!-- http://purl.obolibrary.org/obo/GAZ_00253168 -->

    <owl:NamedIndividual rdf:about="http://purl.obolibrary.org/obo/GAZ_00253168">
        <obo:RO_0001025 rdf:resource="http://purl.obolibrary.org/obo/GAZ_00400000"/>
        <obo:IAO_0000115>A protected area. Established 1982.</obo:IAO_0000115>
        <oboInOwl:hasOBONamespace>GAZ</oboInOwl:hasOBONamespace>
        <oboInOwl:id>GAZ:00253168</oboInOwl:id>
        <rdfs:label>Zangi Nawar Game Reserve</rdfs:label>
    </owl:NamedIndividual>
    


    <!-- http://purl.obolibrary.org/obo/GAZ_00253169 -->

    <owl:NamedIndividual rdf:about="http://purl.obolibrary.org/obo/GAZ_00253169">
        <obo:RO_0001025 rdf:resource="http://purl.obolibrary.org/obo/GAZ_00253168"/>
        <obo:IAO_0000115>A chain of lagoons extending for some 12.8 km along an east-west axis, and is fed by a seasonal stream, the Bohr Lora, rising in the hills to the northeast. The lagoons are separated by sandy ridges and fringed by low bushes.</obo:IAO_0000115>
        <oboInOwl:hasOBONamespace>GAZ</oboInOwl:hasOBONamespace>
        <oboInOwl:id>GAZ:00253169</oboInOwl:id>
        <rdfs:label>Zangi Nawar Lake</rdfs:label>
    </owl:NamedIndividual>
    


    <!-- http://purl.obolibrary.org/obo/GAZ_00253171 -->

    <owl:NamedIndividual rdf:about="http://purl.obolibrary.org/obo/GAZ_00253171">
        <obo:RO_0001025 rdf:resource="http://purl.obolibrary.org/obo/GAZ_00018488"/>
        <obo:IAO_0000115>A seasonal river.</obo:IAO_0000115>
        <oboInOwl:hasOBONamespace>GAZ</oboInOwl:hasOBONamespace>
        <oboInOwl:id>GAZ:00253171</oboInOwl:id>
        <rdfs:label>Akara River</rdfs:label>
    </owl:NamedIndividual>
    


    <!-- http://purl.obolibrary.org/obo/GAZ_00253172 -->

    <owl:NamedIndividual rdf:about="http://purl.obolibrary.org/obo/GAZ_00253172">
        <obo:RO_0001025 rdf:resource="http://purl.obolibrary.org/obo/GAZ_00253171"/>
        <obo:IAO_0000115>A dam. Impounds Akara Reservoir. Located 30 km north of Gwadar Port, Baluchistan.</obo:IAO_0000115>
        <oboInOwl:hasOBONamespace>GAZ</oboInOwl:hasOBONamespace>
        <oboInOwl:id>GAZ:00253172</oboInOwl:id>
        <rdfs:label>Akara Dam</rdfs:label>
    </owl:NamedIndividual>
    


    <!-- http://purl.obolibrary.org/obo/GAZ_00253173 -->

    <owl:NamedIndividual rdf:about="http://purl.obolibrary.org/obo/GAZ_00253173">
        <obo:RO_0001025 rdf:resource="http://purl.obolibrary.org/obo/GAZ_00253171"/>
        <obo:IAO_0000115>A small water storage reservoir. Impounded by Akara Dam. Located 30 km north of Gwadar Port, Baluchistan.</obo:IAO_0000115>
        <oboInOwl:hasOBONamespace>GAZ</oboInOwl:hasOBONamespace>
        <oboInOwl:id>GAZ:00253173</oboInOwl:id>
        <rdfs:label>Akara Reservoir</rdfs:label>
    </owl:NamedIndividual>
    


    <!-- http://purl.obolibrary.org/obo/GAZ_00253174 -->

    <owl:NamedIndividual rdf:about="http://purl.obolibrary.org/obo/GAZ_00253174">
        <obo:RO_0001025 rdf:resource="http://purl.obolibrary.org/obo/GAZ_00018488"/>
        <obo:IAO_0000115>A seasonal river rising in the hills of southwestern Baluchistan and entering the Arabian Sea a few km east of the Iranian border.</obo:IAO_0000115>
        <oboInOwl:hasOBONamespace>GAZ</oboInOwl:hasOBONamespace>
        <oboInOwl:id>GAZ:00253174</oboInOwl:id>
        <rdfs:label>Dasht Kaur</rdfs:label>
    </owl:NamedIndividual>
    


    <!-- http://purl.obolibrary.org/obo/GAZ_00253175 -->

    <owl:NamedIndividual rdf:about="http://purl.obolibrary.org/obo/GAZ_00253175">
        <obo:RO_0001025 rdf:resource="http://purl.obolibrary.org/obo/GAZ_00080188"/>
        <obo:IAO_0000115>A bay.</obo:IAO_0000115>
        <oboInOwl:hasOBONamespace>GAZ</oboInOwl:hasOBONamespace>
        <oboInOwl:id>GAZ:00253175</oboInOwl:id>
        <rdfs:label>Pasni Bay</rdfs:label>
    </owl:NamedIndividual>
    


    <!-- http://purl.obolibrary.org/obo/GAZ_00253177 -->

    <owl:NamedIndividual rdf:about="http://purl.obolibrary.org/obo/GAZ_00253177">
        <obo:RO_0001025 rdf:resource="http://purl.obolibrary.org/obo/GAZ_00400044"/>
        <obo:IAO_0000115>A water storage reservoir. Located southeast of Kohat.</obo:IAO_0000115>
        <oboInOwl:hasOBONamespace>GAZ</oboInOwl:hasOBONamespace>
        <oboInOwl:id>GAZ:00253177</oboInOwl:id>
        <rdfs:label>Kandar Dam</rdfs:label>
    </owl:NamedIndividual>
    


    <!-- http://purl.obolibrary.org/obo/GAZ_00253178 -->

    <owl:NamedIndividual rdf:about="http://purl.obolibrary.org/obo/GAZ_00253178">
        <obo:RO_0001025 rdf:resource="http://purl.obolibrary.org/obo/GAZ_00400031"/>
        <obo:IAO_0000115>A water storage reservoir. Located 40 km east of Peshawar.</obo:IAO_0000115>
        <oboInOwl:hasOBONamespace>GAZ</oboInOwl:hasOBONamespace>
        <oboInOwl:id>GAZ:00253178</oboInOwl:id>
        <rdfs:label>Kheshki Reservoir</rdfs:label>
    </owl:NamedIndividual>
    


    <!-- http://purl.obolibrary.org/obo/GAZ_00253179 -->

    <owl:NamedIndividual rdf:about="http://purl.obolibrary.org/obo/GAZ_00253179">
        <obo:RO_0001025 rdf:resource="http://purl.obolibrary.org/obo/GAZ_00056904"/>
        <obo:IAO_0000115>A brackish lake. Located about 5 km southwest of Chakwal, Punjab.</obo:IAO_0000115>
        <oboInOwl:hasOBONamespace>GAZ</oboInOwl:hasOBONamespace>
        <oboInOwl:id>GAZ:00253179</oboInOwl:id>
        <rdfs:label>Kalar Kahar Lake</rdfs:label>
    </owl:NamedIndividual>
    


    <!-- http://purl.obolibrary.org/obo/GAZ_00253180 -->

    <owl:NamedIndividual rdf:about="http://purl.obolibrary.org/obo/GAZ_00253180">
        <obo:RO_0001025 rdf:resource="http://purl.obolibrary.org/obo/GAZ_00018553"/>
        <obo:IAO_0000115>A protected area. Established 1980.</obo:IAO_0000115>
        <oboInOwl:hasOBONamespace>GAZ</oboInOwl:hasOBONamespace>
        <oboInOwl:id>GAZ:00253180</oboInOwl:id>
        <rdfs:label>Langh Lake Wildlife Sanctuary</rdfs:label>
    </owl:NamedIndividual>
    


    <!-- http://purl.obolibrary.org/obo/GAZ_00253181 -->

    <owl:NamedIndividual rdf:about="http://purl.obolibrary.org/obo/GAZ_00253181">
        <obo:RO_0001025 rdf:resource="http://purl.obolibrary.org/obo/GAZ_00253180"/>
        <obo:IAO_0000115>A former freshwater lake. Now drained.</obo:IAO_0000115>
        <oboInOwl:hasOBONamespace>GAZ</oboInOwl:hasOBONamespace>
        <oboInOwl:id>GAZ:00253181</oboInOwl:id>
        <rdfs:label>Langh Lake</rdfs:label>
    </owl:NamedIndividual>
    


    <!-- http://purl.obolibrary.org/obo/GAZ_00253182 -->

    <owl:NamedIndividual rdf:about="http://purl.obolibrary.org/obo/GAZ_00253182">
        <obo:RO_0001025 rdf:resource="http://purl.obolibrary.org/obo/GAZ_00058456"/>
        <obo:IAO_0000115>A protected area.</obo:IAO_0000115>
        <oboInOwl:hasOBONamespace>GAZ</oboInOwl:hasOBONamespace>
        <oboInOwl:id>GAZ:00253182</oboInOwl:id>
        <rdfs:label>Rawal Lake Game Reserve</rdfs:label>
    </owl:NamedIndividual>
    


    <!-- http://purl.obolibrary.org/obo/GAZ_00253183 -->

    <owl:NamedIndividual rdf:about="http://purl.obolibrary.org/obo/GAZ_00253183">
        <obo:RO_0001025 rdf:resource="http://purl.obolibrary.org/obo/GAZ_00018549"/>
        <obo:IAO_0000115>A protected area. Established 1972-12-20.</obo:IAO_0000115>
        <oboInOwl:hasOBONamespace>GAZ</oboInOwl:hasOBONamespace>
        <oboInOwl:id>GAZ:00253183</oboInOwl:id>
        <rdfs:label>Nara Game Reserve</rdfs:label>
    </owl:NamedIndividual>
    


    <!-- http://purl.obolibrary.org/obo/GAZ_00253185 -->

    <owl:NamedIndividual rdf:about="http://purl.obolibrary.org/obo/GAZ_00253185">
        <obo:RO_0001025 rdf:resource="http://purl.obolibrary.org/obo/GAZ_00400053"/>
        <obo:IAO_0000115>A protected area. Established 1978.</obo:IAO_0000115>
        <oboInOwl:hasOBONamespace>GAZ</oboInOwl:hasOBONamespace>
        <oboInOwl:id>GAZ:00253185</oboInOwl:id>
        <rdfs:label>Head Islam Game Reserve</rdfs:label>
    </owl:NamedIndividual>
    


    <!-- http://purl.obolibrary.org/obo/GAZ_00253186 -->

    <owl:NamedIndividual rdf:about="http://purl.obolibrary.org/obo/GAZ_00253186">
        <obo:RO_0001025 rdf:resource="http://purl.obolibrary.org/obo/GAZ_00080536"/>
        <obo:IAO_0000115>A protected area. Established 1978.</obo:IAO_0000115>
        <oboInOwl:hasOBONamespace>GAZ</oboInOwl:hasOBONamespace>
        <oboInOwl:id>GAZ:00253186</oboInOwl:id>
        <rdfs:label>Head Qadirabad Game Reserve</rdfs:label>
    </owl:NamedIndividual>
    


    <!-- http://purl.obolibrary.org/obo/GAZ_00400000 -->

    <owl:NamedIndividual rdf:about="http://purl.obolibrary.org/obo/GAZ_00400000">
        <obo:RO_0001025 rdf:resource="http://purl.obolibrary.org/obo/GAZ_00005248"/>
        <obo:IAO_0000115>The largest district of Pakistan and is located on the north west corner of Balochistan, Pakistan. It forms a triangular border with Afghanistan and Iran.</obo:IAO_0000115>
        <oboInOwl:hasOBONamespace>GAZ</oboInOwl:hasOBONamespace>
        <oboInOwl:id>GAZ:00400000</oboInOwl:id>
        <rdfs:label>Chagai District</rdfs:label>
    </owl:NamedIndividual>
    


    <!-- http://purl.obolibrary.org/obo/GAZ_00400001 -->

    <owl:NamedIndividual rdf:about="http://purl.obolibrary.org/obo/GAZ_00400001">
        <rdf:type rdf:resource="http://purl.obolibrary.org/obo/ENVO_00000004"/>
        <obo:RO_0001025 rdf:resource="http://purl.obolibrary.org/obo/GAZ_00005248"/>
        <obo:IAO_0000115>A district in the north of Balochistan province of Pakistan. Ziarat district was established in 1986-07.</obo:IAO_0000115>
        <oboInOwl:hasOBONamespace>GAZ</oboInOwl:hasOBONamespace>
        <oboInOwl:id>GAZ:00400001</oboInOwl:id>
        <rdfs:label>Ziarat District</rdfs:label>
    </owl:NamedIndividual>
    


    <!-- http://purl.obolibrary.org/obo/GAZ_00400002 -->

    <owl:NamedIndividual rdf:about="http://purl.obolibrary.org/obo/GAZ_00400002">
        <rdf:type rdf:resource="http://purl.obolibrary.org/obo/ENVO_00000004"/>
        <obo:RO_0001025 rdf:resource="http://purl.obolibrary.org/obo/GAZ_00005248"/>
        <obo:IAO_0000115>A district that lies in the southeast of the Pakistani province of Balochistan.</obo:IAO_0000115>
        <oboInOwl:hasOBONamespace>GAZ</oboInOwl:hasOBONamespace>
        <oboInOwl:id>GAZ:00400002</oboInOwl:id>
        <rdfs:label>Jafarabad District</rdfs:label>
    </owl:NamedIndividual>
    


    <!-- http://purl.obolibrary.org/obo/GAZ_00400003 -->

    <owl:NamedIndividual rdf:about="http://purl.obolibrary.org/obo/GAZ_00400003">
        <rdf:type rdf:resource="http://purl.obolibrary.org/obo/ENVO_00000004"/>
        <obo:RO_0001025 rdf:resource="http://purl.obolibrary.org/obo/GAZ_00005248"/>
        <obo:IAO_0000115>A district in the north-west of the Balochistan province of Pakistan.</obo:IAO_0000115>
        <oboInOwl:hasOBONamespace>GAZ</oboInOwl:hasOBONamespace>
        <oboInOwl:id>GAZ:00400003</oboInOwl:id>
        <rdfs:label>Barkhan District</rdfs:label>
    </owl:NamedIndividual>
    


    <!-- http://purl.obolibrary.org/obo/GAZ_00400004 -->

    <owl:NamedIndividual rdf:about="http://purl.obolibrary.org/obo/GAZ_00400004">
        <obo:RO_0001025 rdf:resource="http://purl.obolibrary.org/obo/GAZ_00005248"/>
        <obo:IAO_0000115>One of the districts of Balochistan province, Pakistan.</obo:IAO_0000115>
        <oboInOwl:hasOBONamespace>GAZ</oboInOwl:hasOBONamespace>
        <oboInOwl:id>GAZ:00400004</oboInOwl:id>
        <rdfs:label>Nushki District</rdfs:label>
    </owl:NamedIndividual>
    


    <!-- http://purl.obolibrary.org/obo/GAZ_00400005 -->

    <owl:NamedIndividual rdf:about="http://purl.obolibrary.org/obo/GAZ_00400005">
        <rdf:type rdf:resource="http://purl.obolibrary.org/obo/ENVO_00000004"/>
        <obo:RO_0001025 rdf:resource="http://purl.obolibrary.org/obo/GAZ_00005248"/>
        <obo:IAO_0000115>A district in the Baluchistan province of Pakistan.</obo:IAO_0000115>
        <oboInOwl:hasOBONamespace>GAZ</oboInOwl:hasOBONamespace>
        <oboInOwl:id>GAZ:00400005</oboInOwl:id>
        <rdfs:label>Sibi District</rdfs:label>
    </owl:NamedIndividual>
    


    <!-- http://purl.obolibrary.org/obo/GAZ_00400006 -->

    <owl:NamedIndividual rdf:about="http://purl.obolibrary.org/obo/GAZ_00400006">
        <rdf:type rdf:resource="http://purl.obolibrary.org/obo/ENVO_00000004"/>
        <obo:RO_0001025 rdf:resource="http://purl.obolibrary.org/obo/GAZ_00005248"/>
        <obo:IAO_0000115>A district in the north-west of Balochistan province of Pakistan. It was part of Quetta Division until the year 2000 when divisions were abolished.</obo:IAO_0000115>
        <oboInOwl:hasOBONamespace>GAZ</oboInOwl:hasOBONamespace>
        <oboInOwl:id>GAZ:00400006</oboInOwl:id>
        <rdfs:label>Quetta District</rdfs:label>
    </owl:NamedIndividual>
    


    <!-- http://purl.obolibrary.org/obo/GAZ_00400007 -->

    <owl:NamedIndividual rdf:about="http://purl.obolibrary.org/obo/GAZ_00400007">
        <obo:RO_0001025 rdf:resource="http://purl.obolibrary.org/obo/GAZ_00005248"/>
        <obo:IAO_0000115>A district is in the centre of Balochistan province of Pakistan. The Bolan area remained under one district Kachhi until 31 1991-12.</obo:IAO_0000115>
        <oboInOwl:hasOBONamespace>GAZ</oboInOwl:hasOBONamespace>
        <oboInOwl:id>GAZ:00400007</oboInOwl:id>
        <rdfs:label>Bolan District</rdfs:label>
    </owl:NamedIndividual>
    


    <!-- http://purl.obolibrary.org/obo/GAZ_00400008 -->

    <owl:NamedIndividual rdf:about="http://purl.obolibrary.org/obo/GAZ_00400008">
        <rdf:type rdf:resource="http://purl.obolibrary.org/obo/ENVO_00000004"/>
        <obo:RO_0001025 rdf:resource="http://purl.obolibrary.org/obo/GAZ_00005248"/>
        <obo:IAO_0000115>A district in the south of the Balochistan province of Pakistan.</obo:IAO_0000115>
        <oboInOwl:hasOBONamespace>GAZ</oboInOwl:hasOBONamespace>
        <oboInOwl:id>GAZ:00400008</oboInOwl:id>
        <rdfs:label>Awaran District</rdfs:label>
    </owl:NamedIndividual>
    


    <!-- http://purl.obolibrary.org/obo/GAZ_00400009 -->

    <owl:NamedIndividual rdf:about="http://purl.obolibrary.org/obo/GAZ_00400009">
        <rdf:type rdf:resource="http://purl.obolibrary.org/obo/ENVO_00000004"/>
        <obo:RO_0001025 rdf:resource="http://purl.obolibrary.org/obo/GAZ_00005248"/>
        <obo:IAO_0000115>A district in the north west of Balochistan province of Pakistan.</obo:IAO_0000115>
        <oboInOwl:hasOBONamespace>GAZ</oboInOwl:hasOBONamespace>
        <oboInOwl:id>GAZ:00400009</oboInOwl:id>
        <rdfs:label>Pishin District</rdfs:label>
    </owl:NamedIndividual>
    


    <!-- http://purl.obolibrary.org/obo/GAZ_00400010 -->

    <owl:NamedIndividual rdf:about="http://purl.obolibrary.org/obo/GAZ_00400010">
        <rdf:type rdf:resource="http://purl.obolibrary.org/obo/ENVO_00000004"/>
        <obo:RO_0001025 rdf:resource="http://purl.obolibrary.org/obo/GAZ_00005248"/>
        <obo:IAO_0000115>A district in the north west of Balochistan province of Pakistan. Zhob district is a Provincially Administered Tribal Area (PATA).</obo:IAO_0000115>
        <oboInOwl:hasOBONamespace>GAZ</oboInOwl:hasOBONamespace>
        <oboInOwl:id>GAZ:00400010</oboInOwl:id>
        <rdfs:label>Zhob District</rdfs:label>
    </owl:NamedIndividual>
    


    <!-- http://purl.obolibrary.org/obo/GAZ_00400011 -->

    <owl:NamedIndividual rdf:about="http://purl.obolibrary.org/obo/GAZ_00400011">
        <obo:RO_0001025 rdf:resource="http://purl.obolibrary.org/obo/GAZ_00005250"/>
        <obo:IAO_0000115>One of the districts in the North-West Frontier Province of Pakistan.</obo:IAO_0000115>
        <oboInOwl:hasOBONamespace>GAZ</oboInOwl:hasOBONamespace>
        <oboInOwl:id>GAZ:00400011</oboInOwl:id>
        <rdfs:label>Malakand District</rdfs:label>
    </owl:NamedIndividual>
    


    <!-- http://purl.obolibrary.org/obo/GAZ_00400012 -->

    <owl:NamedIndividual rdf:about="http://purl.obolibrary.org/obo/GAZ_00400012">
        <obo:RO_0001025 rdf:resource="http://purl.obolibrary.org/obo/GAZ_00005248"/>
        <obo:IAO_0000115>A districy in the south west of Balochistan, province of Pakistan. Kech was notified as a district, with its name as Turbat, on 1977-07-01, when Makran district was given the status of a division and was divided into three districts. Previously it was one of the 3 tehsils of Makran District. In 1995, the name of the district was changed from Turbat to Kech.</obo:IAO_0000115>
        <oboInOwl:hasOBONamespace>GAZ</oboInOwl:hasOBONamespace>
        <oboInOwl:id>GAZ:00400012</oboInOwl:id>
        <rdfs:label>Kech District</rdfs:label>
    </owl:NamedIndividual>
    


    <!-- http://purl.obolibrary.org/obo/GAZ_00400013 -->

    <owl:NamedIndividual rdf:about="http://purl.obolibrary.org/obo/GAZ_00400013">
        <rdf:type rdf:resource="http://purl.obolibrary.org/obo/ENVO_00000004"/>
        <obo:RO_0001025 rdf:resource="http://purl.obolibrary.org/obo/GAZ_00005248"/>
        <obo:IAO_0000115>A district in the centre west of the Pakistani province of Balochistan. Nasirabad&apos;s headquarters are at Dera Murad Jamali.</obo:IAO_0000115>
        <oboInOwl:hasOBONamespace>GAZ</oboInOwl:hasOBONamespace>
        <oboInOwl:id>GAZ:00400013</oboInOwl:id>
        <rdfs:label>Nasirabad District</rdfs:label>
    </owl:NamedIndividual>
    


    <!-- http://purl.obolibrary.org/obo/GAZ_00400014 -->

    <owl:NamedIndividual rdf:about="http://purl.obolibrary.org/obo/GAZ_00400014">
        <rdf:type rdf:resource="http://purl.obolibrary.org/obo/ENVO_00000004"/>
        <obo:RO_0001025 rdf:resource="http://purl.obolibrary.org/obo/GAZ_00005248"/>
        <obo:IAO_0000115>A district in the west of Balochistan province of Pakistan. Panjgur was notified as a district on 1977-07-01 when Makran district was given the status of a division and was divided into three districts. Previously it was one of the 3 tehsils of Makran district.</obo:IAO_0000115>
        <oboInOwl:hasOBONamespace>GAZ</oboInOwl:hasOBONamespace>
        <oboInOwl:id>GAZ:00400014</oboInOwl:id>
        <rdfs:label>Panjgur District</rdfs:label>
    </owl:NamedIndividual>
    


    <!-- http://purl.obolibrary.org/obo/GAZ_00400015 -->

    <owl:NamedIndividual rdf:about="http://purl.obolibrary.org/obo/GAZ_00400015">
        <rdf:type rdf:resource="http://purl.obolibrary.org/obo/ENVO_00000004"/>
        <obo:RO_0001025 rdf:resource="http://purl.obolibrary.org/obo/GAZ_00005248"/>
        <obo:IAO_0000115>A district located in the north west of Balochistan province. Pakistan. Prior to 1991 Mastung was part of Kalat District. For administrative purposes Mastung was separated from Kalat and made a new District in 1991.</obo:IAO_0000115>
        <oboInOwl:hasOBONamespace>GAZ</oboInOwl:hasOBONamespace>
        <oboInOwl:id>GAZ:00400015</oboInOwl:id>
        <rdfs:label>Mastung District</rdfs:label>
    </owl:NamedIndividual>
    


    <!-- http://purl.obolibrary.org/obo/GAZ_00400016 -->

    <owl:NamedIndividual rdf:about="http://purl.obolibrary.org/obo/GAZ_00400016">
        <rdf:type rdf:resource="http://purl.obolibrary.org/obo/ENVO_00000004"/>
        <obo:RO_0001025 rdf:resource="http://purl.obolibrary.org/obo/GAZ_00005248"/>
        <obo:IAO_0000115>A district in the centre of Balochistan province of Pakistan. Loralai district was created on 1903-10. Loralai town is the district headquarters. Loralai was further partitioned in 1992 when Musakhel and Barkhan were given the status of separate administrative districts.</obo:IAO_0000115>
        <oboInOwl:hasOBONamespace>GAZ</oboInOwl:hasOBONamespace>
        <oboInOwl:id>GAZ:00400016</oboInOwl:id>
        <rdfs:label>Loralai District</rdfs:label>
    </owl:NamedIndividual>
    


    <!-- http://purl.obolibrary.org/obo/GAZ_00400017 -->

    <owl:NamedIndividual rdf:about="http://purl.obolibrary.org/obo/GAZ_00400017">
        <rdf:type rdf:resource="http://purl.obolibrary.org/obo/ENVO_00000004"/>
        <obo:RO_0001025 rdf:resource="http://purl.obolibrary.org/obo/GAZ_00005248"/>
        <obo:IAO_0000115>A district in Balochistan, Pakistan.</obo:IAO_0000115>
        <oboInOwl:hasOBONamespace>GAZ</oboInOwl:hasOBONamespace>
        <oboInOwl:id>GAZ:00400017</oboInOwl:id>
        <rdfs:label>Kalat District</rdfs:label>
    </owl:NamedIndividual>
    


    <!-- http://purl.obolibrary.org/obo/GAZ_00400018 -->

    <owl:NamedIndividual rdf:about="http://purl.obolibrary.org/obo/GAZ_00400018">
        <rdf:type rdf:resource="http://purl.obolibrary.org/obo/ENVO_00000004"/>
        <obo:RO_0001025 rdf:resource="http://purl.obolibrary.org/obo/GAZ_00005248"/>
        <obo:IAO_0000115>A district located in the centre of Balochistan province of Pakistan. Khuzdar is the capital of Khuzdar district.</obo:IAO_0000115>
        <oboInOwl:hasOBONamespace>GAZ</oboInOwl:hasOBONamespace>
        <oboInOwl:id>GAZ:00400018</oboInOwl:id>
        <rdfs:label>Khuzdar District</rdfs:label>
    </owl:NamedIndividual>
    


    <!-- http://purl.obolibrary.org/obo/GAZ_00400019 -->

    <owl:NamedIndividual rdf:about="http://purl.obolibrary.org/obo/GAZ_00400019">
        <rdf:type rdf:resource="http://purl.obolibrary.org/obo/ENVO_00000004"/>
        <obo:RO_0001025 rdf:resource="http://purl.obolibrary.org/obo/GAZ_00005248"/>
        <obo:IAO_0000115>A district in the north west of Balochistan province of Pakistan. Musakhel was notified as a district on 1992-01-01 when Loralai District was divided into three districts, named Musakhel, Barkhan, and Loralai. Previously, Musakhel was one of the 4 sub-divisions of Loralai district.</obo:IAO_0000115>
        <oboInOwl:hasOBONamespace>GAZ</oboInOwl:hasOBONamespace>
        <oboInOwl:id>GAZ:00400019</oboInOwl:id>
        <rdfs:label>Musakhel District</rdfs:label>
    </owl:NamedIndividual>
    


    <!-- http://purl.obolibrary.org/obo/GAZ_00400020 -->

    <owl:NamedIndividual rdf:about="http://purl.obolibrary.org/obo/GAZ_00400020">
        <obo:RO_0001025 rdf:resource="http://purl.obolibrary.org/obo/GAZ_00005248"/>
        <obo:IAO_0000115>A coastal district of Balochistan province of Pakistan. It became a separate district in Kalat division on 1954-06-30.</obo:IAO_0000115>
        <oboInOwl:hasOBONamespace>GAZ</oboInOwl:hasOBONamespace>
        <oboInOwl:id>GAZ:00400020</oboInOwl:id>
        <rdfs:label>Lasbela District</rdfs:label>
    </owl:NamedIndividual>
    


    <!-- http://purl.obolibrary.org/obo/GAZ_00400021 -->

    <owl:NamedIndividual rdf:about="http://purl.obolibrary.org/obo/GAZ_00400021">
        <rdf:type rdf:resource="http://purl.obolibrary.org/obo/ENVO_00000004"/>
        <obo:RO_0001025 rdf:resource="http://purl.obolibrary.org/obo/GAZ_00005248"/>
        <obo:IAO_0000115>A district located in the south west of Balochistan province of Pakistan.</obo:IAO_0000115>
        <oboInOwl:hasOBONamespace>GAZ</oboInOwl:hasOBONamespace>
        <oboInOwl:id>GAZ:00400021</oboInOwl:id>
        <rdfs:label>Dera Bugti District</rdfs:label>
    </owl:NamedIndividual>
    


    <!-- http://purl.obolibrary.org/obo/GAZ_00400022 -->

    <owl:NamedIndividual rdf:about="http://purl.obolibrary.org/obo/GAZ_00400022">
        <rdf:type rdf:resource="http://purl.obolibrary.org/obo/ENVO_00000004"/>
        <obo:RO_0001025 rdf:resource="http://purl.obolibrary.org/obo/GAZ_00005248"/>
        <obo:IAO_0000115>A district in the centre of Balochistan province of Pakistan.</obo:IAO_0000115>
        <oboInOwl:hasOBONamespace>GAZ</oboInOwl:hasOBONamespace>
        <oboInOwl:id>GAZ:00400022</oboInOwl:id>
        <rdfs:label>Jhal Magsi District</rdfs:label>
    </owl:NamedIndividual>
    


    <!-- http://purl.obolibrary.org/obo/GAZ_00400023 -->

    <owl:NamedIndividual rdf:about="http://purl.obolibrary.org/obo/GAZ_00400023">
        <rdf:type rdf:resource="http://purl.obolibrary.org/obo/ENVO_00000004"/>
        <obo:RO_0001025 rdf:resource="http://purl.obolibrary.org/obo/GAZ_00005248"/>
        <obo:IAO_0000115>A district in the Balochistan province in Pakistan. It is bounded in the north by Loralai District, Dera Bugti in the south, in the east Rojhan-Mazari and Sibi District in the west.</obo:IAO_0000115>
        <oboInOwl:hasOBONamespace>GAZ</oboInOwl:hasOBONamespace>
        <oboInOwl:id>GAZ:00400023</oboInOwl:id>
        <rdfs:label>Kohlu District</rdfs:label>
    </owl:NamedIndividual>
    


    <!-- http://purl.obolibrary.org/obo/GAZ_00400024 -->

    <owl:NamedIndividual rdf:about="http://purl.obolibrary.org/obo/GAZ_00400024">
        <rdf:type rdf:resource="http://purl.obolibrary.org/obo/ENVO_00000004"/>
        <obo:RO_0001025 rdf:resource="http://purl.obolibrary.org/obo/GAZ_00005248"/>
        <obo:IAO_0000115>A district in the north west of Balochistan province of Pakistan. Qilla Saifullah became a district on 1988-12-14.</obo:IAO_0000115>
        <oboInOwl:hasOBONamespace>GAZ</oboInOwl:hasOBONamespace>
        <oboInOwl:id>GAZ:00400024</oboInOwl:id>
        <rdfs:label>Qilla Saifullah District</rdfs:label>
    </owl:NamedIndividual>
    


    <!-- http://purl.obolibrary.org/obo/GAZ_00400025 -->

    <owl:NamedIndividual rdf:about="http://purl.obolibrary.org/obo/GAZ_00400025">
        <rdf:type rdf:resource="http://purl.obolibrary.org/obo/ENVO_00000004"/>
        <obo:RO_0001025 rdf:resource="http://purl.obolibrary.org/obo/GAZ_00005248"/>
        <obo:IAO_0000115>A district in the north-west of Balochistan province of Pakistan.</obo:IAO_0000115>
        <oboInOwl:hasOBONamespace>GAZ</oboInOwl:hasOBONamespace>
        <oboInOwl:id>GAZ:00400025</oboInOwl:id>
        <rdfs:label>Kharan District</rdfs:label>
    </owl:NamedIndividual>
    


    <!-- http://purl.obolibrary.org/obo/GAZ_00400026 -->

    <owl:NamedIndividual rdf:about="http://purl.obolibrary.org/obo/GAZ_00400026">
        <rdf:type rdf:resource="http://purl.obolibrary.org/obo/ENVO_00000004"/>
        <obo:RO_0001025 rdf:resource="http://purl.obolibrary.org/obo/GAZ_00005248"/>
        <obo:IAO_0000115>A district in the north west of Balochistan province of Pakistan. Killa Abdullah was separated from Pishin District and made a new district in 1993-06.</obo:IAO_0000115>
        <oboInOwl:hasOBONamespace>GAZ</oboInOwl:hasOBONamespace>
        <oboInOwl:id>GAZ:00400026</oboInOwl:id>
        <rdfs:label>Qilla Abdullah District</rdfs:label>
    </owl:NamedIndividual>
    


    <!-- http://purl.obolibrary.org/obo/GAZ_00400027 -->

    <owl:NamedIndividual rdf:about="http://purl.obolibrary.org/obo/GAZ_00400027">
        <rdf:type rdf:resource="http://purl.obolibrary.org/obo/ENVO_00000004"/>
        <obo:RO_0001025 rdf:resource="http://purl.obolibrary.org/obo/GAZ_00005250"/>
        <obo:IAO_0000115>A district in the North-West Frontier Province of Pakistan, which contains the town of Mansehra and the Kaghan Valley.</obo:IAO_0000115>
        <oboInOwl:hasOBONamespace>GAZ</oboInOwl:hasOBONamespace>
        <oboInOwl:id>GAZ:00400027</oboInOwl:id>
        <rdfs:label>Mansehra District</rdfs:label>
    </owl:NamedIndividual>
    


    <!-- http://purl.obolibrary.org/obo/GAZ_00400028 -->

    <owl:NamedIndividual rdf:about="http://purl.obolibrary.org/obo/GAZ_00400028">
        <rdf:type rdf:resource="http://purl.obolibrary.org/obo/ENVO_00000004"/>
        <obo:RO_0001025 rdf:resource="http://purl.obolibrary.org/obo/GAZ_00005250"/>
        <obo:IAO_0000115>A district of North West Frontier Province of Pakistan.</obo:IAO_0000115>
        <oboInOwl:hasOBONamespace>GAZ</oboInOwl:hasOBONamespace>
        <oboInOwl:id>GAZ:00400028</oboInOwl:id>
        <rdfs:label>Dir Lower District</rdfs:label>
    </owl:NamedIndividual>
    


    <!-- http://purl.obolibrary.org/obo/GAZ_00400029 -->

    <owl:NamedIndividual rdf:about="http://purl.obolibrary.org/obo/GAZ_00400029">
        <rdf:type rdf:resource="http://purl.obolibrary.org/obo/ENVO_00000004"/>
        <obo:RO_0001025 rdf:resource="http://purl.obolibrary.org/obo/GAZ_00005250"/>
        <obo:IAO_0000115>A district in the North-West Frontier Province of Pakistan.</obo:IAO_0000115>
        <oboInOwl:hasOBONamespace>GAZ</oboInOwl:hasOBONamespace>
        <oboInOwl:id>GAZ:00400029</oboInOwl:id>
        <rdfs:label>Shangla District</rdfs:label>
    </owl:NamedIndividual>
    


    <!-- http://purl.obolibrary.org/obo/GAZ_00400030 -->

    <owl:NamedIndividual rdf:about="http://purl.obolibrary.org/obo/GAZ_00400030">
        <rdf:type rdf:resource="http://purl.obolibrary.org/obo/ENVO_00000004"/>
        <obo:RO_0001025 rdf:resource="http://purl.obolibrary.org/obo/GAZ_00005250"/>
        <obo:IAO_0000115>A district of North West Frontier Province of Pakistan.</obo:IAO_0000115>
        <oboInOwl:hasOBONamespace>GAZ</oboInOwl:hasOBONamespace>
        <oboInOwl:id>GAZ:00400030</oboInOwl:id>
        <rdfs:label>Dir Upper District</rdfs:label>
    </owl:NamedIndividual>
    


    <!-- http://purl.obolibrary.org/obo/GAZ_00400031 -->

    <owl:NamedIndividual rdf:about="http://purl.obolibrary.org/obo/GAZ_00400031">
        <rdf:type rdf:resource="http://purl.obolibrary.org/obo/ENVO_00000004"/>
        <obo:RO_0001025 rdf:resource="http://purl.obolibrary.org/obo/GAZ_00005250"/>
        <obo:IAO_0000115>A district in the North-West Frontier Province of Pakistan.</obo:IAO_0000115>
        <oboInOwl:hasOBONamespace>GAZ</oboInOwl:hasOBONamespace>
        <oboInOwl:id>GAZ:00400031</oboInOwl:id>
        <rdfs:label>Peshawar District</rdfs:label>
    </owl:NamedIndividual>
    


    <!-- http://purl.obolibrary.org/obo/GAZ_00400032 -->

    <owl:NamedIndividual rdf:about="http://purl.obolibrary.org/obo/GAZ_00400032">
        <rdf:type rdf:resource="http://purl.obolibrary.org/obo/ENVO_00000004"/>
        <obo:RO_0001025 rdf:resource="http://purl.obolibrary.org/obo/GAZ_00005250"/>
        <obo:IAO_0000115>A district in the North-West Frontier Province (NWFP) of Pakistan. The capital is Saidu Sharif.</obo:IAO_0000115>
        <oboInOwl:hasOBONamespace>GAZ</oboInOwl:hasOBONamespace>
        <oboInOwl:id>GAZ:00400032</oboInOwl:id>
        <rdfs:label>Swat District</rdfs:label>
    </owl:NamedIndividual>
    


    <!-- http://purl.obolibrary.org/obo/GAZ_00400033 -->

    <owl:NamedIndividual rdf:about="http://purl.obolibrary.org/obo/GAZ_00400033">
        <rdf:type rdf:resource="http://purl.obolibrary.org/obo/ENVO_00000004"/>
        <obo:RO_0001025 rdf:resource="http://purl.obolibrary.org/obo/GAZ_00005250"/>
        <obo:IAO_0000115>A district that lies between the Indus and Kabul rivers, in the North-West Frontier Province of Pakistan.</obo:IAO_0000115>
        <oboInOwl:hasOBONamespace>GAZ</oboInOwl:hasOBONamespace>
        <oboInOwl:id>GAZ:00400033</oboInOwl:id>
        <rdfs:label>Swabi District</rdfs:label>
    </owl:NamedIndividual>
    


    <!-- http://purl.obolibrary.org/obo/GAZ_00400034 -->

    <owl:NamedIndividual rdf:about="http://purl.obolibrary.org/obo/GAZ_00400034">
        <rdf:type rdf:resource="http://purl.obolibrary.org/obo/ENVO_00000004"/>
        <obo:RO_0001025 rdf:resource="http://purl.obolibrary.org/obo/GAZ_00005250"/>
        <obo:IAO_0000115>A district in the North-West Frontier Province of Pakistan, the city of Tank is the capital of the district. Tank was formerly part of Dera Ismail Khan District. Tank is bounded by the districts of Lakki Marwat to the northeast, Dera Ismail Khan to the east and southeast, and South Waziristan to the southwest, west, and northwest.</obo:IAO_0000115>
        <oboInOwl:hasOBONamespace>GAZ</oboInOwl:hasOBONamespace>
        <oboInOwl:id>GAZ:00400034</oboInOwl:id>
        <rdfs:label>Tank District</rdfs:label>
    </owl:NamedIndividual>
    


    <!-- http://purl.obolibrary.org/obo/GAZ_00400035 -->

    <owl:NamedIndividual rdf:about="http://purl.obolibrary.org/obo/GAZ_00400035">
        <rdf:type rdf:resource="http://purl.obolibrary.org/obo/ENVO_00000004"/>
        <obo:RO_0001025 rdf:resource="http://purl.obolibrary.org/obo/GAZ_00005250"/>
        <obo:IAO_0000115>A district in the North-West Frontier Province of Pakistan that contains the city of Mardan.</obo:IAO_0000115>
        <oboInOwl:hasOBONamespace>GAZ</oboInOwl:hasOBONamespace>
        <oboInOwl:id>GAZ:00400035</oboInOwl:id>
        <rdfs:label>Mardan District</rdfs:label>
    </owl:NamedIndividual>
    


    <!-- http://purl.obolibrary.org/obo/GAZ_00400036 -->

    <owl:NamedIndividual rdf:about="http://purl.obolibrary.org/obo/GAZ_00400036">
        <rdf:type rdf:resource="http://purl.obolibrary.org/obo/ENVO_00000004"/>
        <obo:RO_0001025 rdf:resource="http://purl.obolibrary.org/obo/GAZ_00005250"/>
        <obo:IAO_0000115>A district in the North-West Frontier Province of Pakistan; the principal city is Nowshera.</obo:IAO_0000115>
        <oboInOwl:hasOBONamespace>GAZ</oboInOwl:hasOBONamespace>
        <oboInOwl:id>GAZ:00400036</oboInOwl:id>
        <rdfs:label>Nowshera District</rdfs:label>
    </owl:NamedIndividual>
    


    <!-- http://purl.obolibrary.org/obo/GAZ_00400037 -->

    <owl:NamedIndividual rdf:about="http://purl.obolibrary.org/obo/GAZ_00400037">
        <obo:RO_0001025 rdf:resource="http://purl.obolibrary.org/obo/GAZ_00005250"/>
        <obo:IAO_0000115>One of the Southern Districts of North-West Frontier Province in Pakistan. It was created as an administrative district on 1992-07-01, prior to which it was a Tehsil of Bannu District.</obo:IAO_0000115>
        <oboInOwl:hasOBONamespace>GAZ</oboInOwl:hasOBONamespace>
        <oboInOwl:id>GAZ:00400037</oboInOwl:id>
        <rdfs:label>Lakki Marwat District</rdfs:label>
    </owl:NamedIndividual>
    


    <!-- http://purl.obolibrary.org/obo/GAZ_00400038 -->

    <owl:NamedIndividual rdf:about="http://purl.obolibrary.org/obo/GAZ_00400038">
        <rdf:type rdf:resource="http://purl.obolibrary.org/obo/ENVO_00000004"/>
        <obo:RO_0001025 rdf:resource="http://purl.obolibrary.org/obo/GAZ_00005250"/>
        <obo:IAO_0000115>A district located in what used to be the Hazara Division of NWFP, Pakistan. Batgram obtained the status of district in 1993-07 when it was upgraded from a Tehsil and separated from Mansehra District by an executive order. It has geographical borders with Kohistan District, Tribal Area of Kala Dhaka (Black Mountain of Hazara), Shangla District and Malakand Division.</obo:IAO_0000115>
        <oboInOwl:hasOBONamespace>GAZ</oboInOwl:hasOBONamespace>
        <oboInOwl:id>GAZ:00400038</oboInOwl:id>
        <rdfs:label>Batagram District</rdfs:label>
    </owl:NamedIndividual>
    


    <!-- http://purl.obolibrary.org/obo/GAZ_00400039 -->

    <owl:NamedIndividual rdf:about="http://purl.obolibrary.org/obo/GAZ_00400039">
        <obo:RO_0001025 rdf:resource="http://purl.obolibrary.org/obo/GAZ_00005250"/>
        <obo:IAO_0000115>One of the 24 districts in the North-West Frontier Province of Pakistan, the capital of the district is the town of Dera Ismail Khan. The district of Dera Ismail Khan is bounded on the east by Punjab Province, to the southwest by South Waziristan district, and to the northwest by Tank and Lakki Marwat districts.</obo:IAO_0000115>
        <oboInOwl:hasOBONamespace>GAZ</oboInOwl:hasOBONamespace>
        <oboInOwl:id>GAZ:00400039</oboInOwl:id>
        <rdfs:label>Dera Ismail Khan District</rdfs:label>
    </owl:NamedIndividual>
    


    <!-- http://purl.obolibrary.org/obo/GAZ_00400040 -->

    <owl:NamedIndividual rdf:about="http://purl.obolibrary.org/obo/GAZ_00400040">
        <rdf:type rdf:resource="http://purl.obolibrary.org/obo/ENVO_00000004"/>
        <obo:RO_0001025 rdf:resource="http://purl.obolibrary.org/obo/GAZ_00005250"/>
        <obo:IAO_0000115>A district of the North-West Frontier Province of Pakistan.</obo:IAO_0000115>
        <oboInOwl:hasOBONamespace>GAZ</oboInOwl:hasOBONamespace>
        <oboInOwl:id>GAZ:00400040</oboInOwl:id>
        <rdfs:label>Kohistan District</rdfs:label>
    </owl:NamedIndividual>
    


    <!-- http://purl.obolibrary.org/obo/GAZ_00400041 -->

    <owl:NamedIndividual rdf:about="http://purl.obolibrary.org/obo/GAZ_00400041">
        <rdf:type rdf:resource="http://purl.obolibrary.org/obo/ENVO_00000004"/>
        <obo:RO_0001025 rdf:resource="http://purl.obolibrary.org/obo/GAZ_00005250"/>
        <obo:IAO_0000115>A district in Hazara Division in the North-West Frontier Province (NWFP) of Pakistan that contains the city of Haripur, located on the bank of a stream called Dor. The District of Haripur was a Tehsil of Abbottabad District until 1992 when it was separated from the District of Abbottabad and made into a district in its own right.</obo:IAO_0000115>
        <oboInOwl:hasOBONamespace>GAZ</oboInOwl:hasOBONamespace>
        <oboInOwl:id>GAZ:00400041</oboInOwl:id>
        <rdfs:label>Haripur District</rdfs:label>
    </owl:NamedIndividual>
    


    <!-- http://purl.obolibrary.org/obo/GAZ_00400042 -->

    <owl:NamedIndividual rdf:about="http://purl.obolibrary.org/obo/GAZ_00400042">
        <rdf:type rdf:resource="http://purl.obolibrary.org/obo/ENVO_00000004"/>
        <obo:RO_0001025 rdf:resource="http://purl.obolibrary.org/obo/GAZ_00005250"/>
        <obo:IAO_0000115>A district in the North-West Frontier Province of Pakistan. Abbottabad is the principal town of this district. Neighbouring districts are Mansehra to the North, Muzaffarabad to the east, Haripur to the west, and Rawalpindi to the South.</obo:IAO_0000115>
        <oboInOwl:hasOBONamespace>GAZ</oboInOwl:hasOBONamespace>
        <oboInOwl:id>GAZ:00400042</oboInOwl:id>
        <rdfs:label>Abbottabad District</rdfs:label>
    </owl:NamedIndividual>
    


    <!-- http://purl.obolibrary.org/obo/GAZ_00400043 -->

    <owl:NamedIndividual rdf:about="http://purl.obolibrary.org/obo/GAZ_00400043">
        <rdf:type rdf:resource="http://purl.obolibrary.org/obo/ENVO_00000004"/>
        <obo:RO_0001025 rdf:resource="http://purl.obolibrary.org/obo/GAZ_00005250"/>
        <obo:IAO_0000115>A district in the North-West Frontier Province of Pakistan that contains the town of Charsadda. Charsadda is located in the west of the NWFP and is bounded by Malakand District on the north. Mardan district on the east, Nowshera and Peshawar districts on the south and the Mohmand Agency of the Federally Administered Tribal Areas on the west.</obo:IAO_0000115>
        <oboInOwl:hasOBONamespace>GAZ</oboInOwl:hasOBONamespace>
        <oboInOwl:id>GAZ:00400043</oboInOwl:id>
        <rdfs:label>Charsadda District</rdfs:label>
    </owl:NamedIndividual>
    


    <!-- http://purl.obolibrary.org/obo/GAZ_00400044 -->

    <owl:NamedIndividual rdf:about="http://purl.obolibrary.org/obo/GAZ_00400044">
        <rdf:type rdf:resource="http://purl.obolibrary.org/obo/ENVO_00000004"/>
        <obo:RO_0001025 rdf:resource="http://purl.obolibrary.org/obo/GAZ_00005250"/>
        <obo:IAO_0000115>A district of the North-West Frontier Province of Pakistan, Kohat city is the capital of the district.</obo:IAO_0000115>
        <oboInOwl:hasOBONamespace>GAZ</oboInOwl:hasOBONamespace>
        <oboInOwl:id>GAZ:00400044</oboInOwl:id>
        <rdfs:label>Kohat District</rdfs:label>
    </owl:NamedIndividual>
    


    <!-- http://purl.obolibrary.org/obo/GAZ_00400045 -->

    <owl:NamedIndividual rdf:about="http://purl.obolibrary.org/obo/GAZ_00400045">
        <rdf:type rdf:resource="http://purl.obolibrary.org/obo/ENVO_00000004"/>
        <obo:RO_0001025 rdf:resource="http://purl.obolibrary.org/obo/GAZ_00005250"/>
        <obo:IAO_0000115>A district in the North-West Frontier Province of Pakistan that contains the town of Chitral. Chitral District is the most northern district in the North West Frontier Province, to the west and north is Afghanistan - in the north the Wakhan Corridor, a narrow strip of Afghanistan, separates Pakistan from Tajikstan. To the east of Chitral are the Northern Areas and to the south are the districts of Upper Dir and Swat.</obo:IAO_0000115>
        <oboInOwl:hasOBONamespace>GAZ</oboInOwl:hasOBONamespace>
        <oboInOwl:id>GAZ:00400045</oboInOwl:id>
        <rdfs:label>Chitral District</rdfs:label>
    </owl:NamedIndividual>
    


    <!-- http://purl.obolibrary.org/obo/GAZ_00400046 -->

    <owl:NamedIndividual rdf:about="http://purl.obolibrary.org/obo/GAZ_00400046">
        <obo:RO_0001025 rdf:resource="http://purl.obolibrary.org/obo/GAZ_00005250"/>
        <obo:IAO_0000115>One of the twenty four districts of the North-West Frontier Province of Pakistan. It is bounded by the districts of Karak, Lakki Marwat and the North, South Wazirestan Agencies.</obo:IAO_0000115>
        <oboInOwl:hasOBONamespace>GAZ</oboInOwl:hasOBONamespace>
        <oboInOwl:id>GAZ:00400046</oboInOwl:id>
        <rdfs:label>Bannu District</rdfs:label>
    </owl:NamedIndividual>
    


    <!-- http://purl.obolibrary.org/obo/GAZ_00400047 -->

    <owl:NamedIndividual rdf:about="http://purl.obolibrary.org/obo/GAZ_00400047">
        <rdf:type rdf:resource="http://purl.obolibrary.org/obo/ENVO_00000004"/>
        <obo:RO_0001025 rdf:resource="http://purl.obolibrary.org/obo/GAZ_00005250"/>
        <obo:IAO_0000115>A district in the Northwest Frontier Province of Pakistan. Until 1998 Hangu was part of Kohat District but afterwards became a district itself. Its area starts from a village named Khawaja Khizer (Jawzara) which is the boundary between Kohat and Hangu Districts.</obo:IAO_0000115>
        <oboInOwl:hasOBONamespace>GAZ</oboInOwl:hasOBONamespace>
        <oboInOwl:id>GAZ:00400047</oboInOwl:id>
        <rdfs:label>Hangu District</rdfs:label>
    </owl:NamedIndividual>
    


    <!-- http://purl.obolibrary.org/obo/GAZ_00400048 -->

    <owl:NamedIndividual rdf:about="http://purl.obolibrary.org/obo/GAZ_00400048">
        <rdf:type rdf:resource="http://purl.obolibrary.org/obo/ENVO_00000004"/>
        <obo:RO_0001025 rdf:resource="http://purl.obolibrary.org/obo/GAZ_00005250"/>
        <obo:IAO_0000115>A district of the North-West Frontier Province, Pakistan. It is situated to the south of Kohat District and on the north side of Bannu and Lakki Marwat districts on the main Indus Highway between Peshawar and Karachi - it is 123 km from the provincial capital Peshawar.</obo:IAO_0000115>
        <oboInOwl:hasOBONamespace>GAZ</oboInOwl:hasOBONamespace>
        <oboInOwl:id>GAZ:00400048</oboInOwl:id>
        <rdfs:label>Karak District</rdfs:label>
    </owl:NamedIndividual>
    


    <!-- http://purl.obolibrary.org/obo/GAZ_00400049 -->

    <owl:NamedIndividual rdf:about="http://purl.obolibrary.org/obo/GAZ_00400049">
        <rdf:type rdf:resource="http://purl.obolibrary.org/obo/ENVO_00000004"/>
        <obo:RO_0001025 rdf:resource="http://purl.obolibrary.org/obo/GAZ_00005250"/>
        <obo:IAO_0000115>A district of the North West Frontier Province of Pakistan. Until 2000 it was a part of Malakand Division - until this district was abolished.</obo:IAO_0000115>
        <oboInOwl:hasOBONamespace>GAZ</oboInOwl:hasOBONamespace>
        <oboInOwl:id>GAZ:00400049</oboInOwl:id>
        <rdfs:label>Buner District</rdfs:label>
    </owl:NamedIndividual>
    


    <!-- http://purl.obolibrary.org/obo/GAZ_00400050 -->

    <owl:NamedIndividual rdf:about="http://purl.obolibrary.org/obo/GAZ_00400050">
        <obo:RO_0001025 rdf:resource="http://purl.obolibrary.org/obo/GAZ_00005249"/>
        <obo:IAO_0000115>A District of Punjab province in Pakistan.</obo:IAO_0000115>
        <oboInOwl:hasOBONamespace>GAZ</oboInOwl:hasOBONamespace>
        <oboInOwl:id>GAZ:00400050</oboInOwl:id>
        <rdfs:label>Rajanpur District</rdfs:label>
    </owl:NamedIndividual>
    


    <!-- http://purl.obolibrary.org/obo/GAZ_00400051 -->

    <owl:NamedIndividual rdf:about="http://purl.obolibrary.org/obo/GAZ_00400051">
        <obo:RO_0001025 rdf:resource="http://purl.obolibrary.org/obo/GAZ_00005249"/>
        <obo:IAO_0000115>One of the districts in the province of Punjab, Pakistan. Narowal city is the capital of the district. The district is bounded on the northwest by Sialkot District, on the north by Kashmir, on the east by Gurdaspur district (India) which contains the Pathankot tehsil contiguous to Pakistan; and internationalised on the south by Amritsar district (India) and Sheikhupura district.</obo:IAO_0000115>
        <oboInOwl:hasOBONamespace>GAZ</oboInOwl:hasOBONamespace>
        <oboInOwl:id>GAZ:00400051</oboInOwl:id>
        <rdfs:label>Narowal District</rdfs:label>
    </owl:NamedIndividual>
    


    <!-- http://purl.obolibrary.org/obo/GAZ_00400052 -->

    <owl:NamedIndividual rdf:about="http://purl.obolibrary.org/obo/GAZ_00400052">
        <rdf:type rdf:resource="http://purl.obolibrary.org/obo/ENVO_00000004"/>
        <obo:RO_0001025 rdf:resource="http://purl.obolibrary.org/obo/GAZ_00005249"/>
        <obo:IAO_0000115>A district of Pakistan, Pakistan - the capital city is Vehari. The district was created in 1976 out of the three tehsils of Multan District (Vehari, Burewala and Mailsi). Location of Vehari, highlighted in red, within Punjab. The district borders with Bahawalnagar and Bahawalpur on the southern side, with Pakpattan on the eastern, with Khanewal and Lodhran on western and with Sahiwal and Khanewal on northern side.</obo:IAO_0000115>
        <oboInOwl:hasOBONamespace>GAZ</oboInOwl:hasOBONamespace>
        <oboInOwl:id>GAZ:00400052</oboInOwl:id>
        <rdfs:label>Vehari District</rdfs:label>
    </owl:NamedIndividual>
    


    <!-- http://purl.obolibrary.org/obo/GAZ_00400053 -->

    <owl:NamedIndividual rdf:about="http://purl.obolibrary.org/obo/GAZ_00400053">
        <obo:RO_0001025 rdf:resource="http://purl.obolibrary.org/obo/GAZ_00005249"/>
        <obo:IAO_0000115>A District in the Punjab province of Pakistan. Multan District is surrounded by the Khanewal District to the North and North East, the Vehari District to the East and Lodhran District to the South. The Chenab River passes on its Western side, across which lies Muzaffargarh District.</obo:IAO_0000115>
        <oboInOwl:hasOBONamespace>GAZ</oboInOwl:hasOBONamespace>
        <oboInOwl:id>GAZ:00400053</oboInOwl:id>
        <rdfs:label>Multan District</rdfs:label>
    </owl:NamedIndividual>
    


    <!-- http://purl.obolibrary.org/obo/GAZ_00400054 -->

    <owl:NamedIndividual rdf:about="http://purl.obolibrary.org/obo/GAZ_00400054">
        <rdf:type rdf:resource="http://purl.obolibrary.org/obo/ENVO_00000004"/>
        <obo:RO_0001025 rdf:resource="http://purl.obolibrary.org/obo/GAZ_00005249"/>
        <obo:IAO_0000115>A district in the Punjab province of Pakistan. Nankana Sahib is principle town of the district. The district, formerly part of Sheikhupura District, was created in 2005.</obo:IAO_0000115>
        <oboInOwl:hasOBONamespace>GAZ</oboInOwl:hasOBONamespace>
        <oboInOwl:id>GAZ:00400054</oboInOwl:id>
        <rdfs:label>Nankana Sahib District</rdfs:label>
    </owl:NamedIndividual>
    


    <!-- http://purl.obolibrary.org/obo/GAZ_00400055 -->

    <owl:NamedIndividual rdf:about="http://purl.obolibrary.org/obo/GAZ_00400055">
        <rdf:type rdf:resource="http://purl.obolibrary.org/obo/ENVO_00000004"/>
        <obo:RO_0001025 rdf:resource="http://purl.obolibrary.org/obo/GAZ_00005249"/>
        <obo:IAO_0000115>A district of Punjab, Pakistan. It is located on Multan Road some 110 km from Lahore.</obo:IAO_0000115>
        <oboInOwl:hasOBONamespace>GAZ</oboInOwl:hasOBONamespace>
        <oboInOwl:id>GAZ:00400055</oboInOwl:id>
        <rdfs:label>Okara District</rdfs:label>
    </owl:NamedIndividual>
    


    <!-- http://purl.obolibrary.org/obo/GAZ_00400056 -->

    <owl:NamedIndividual rdf:about="http://purl.obolibrary.org/obo/GAZ_00400056">
        <obo:RO_0001025 rdf:resource="http://purl.obolibrary.org/obo/GAZ_00005249"/>
        <obo:IAO_0000115>A District in the north-west of Punjab province, Pakistan. It borders Lakki Marwat district in the west, Kohat and Karak districts in the North west and Dera Ismail Khan District in the southwest. Attock lies in the north, Chakwal in the north east, Khushab in the east and Bhakkar in the south.</obo:IAO_0000115>
        <oboInOwl:hasOBONamespace>GAZ</oboInOwl:hasOBONamespace>
        <oboInOwl:id>GAZ:00400056</oboInOwl:id>
        <rdfs:label>Mianwali District</rdfs:label>
    </owl:NamedIndividual>
    


    <!-- http://purl.obolibrary.org/obo/GAZ_00400057 -->

    <owl:NamedIndividual rdf:about="http://purl.obolibrary.org/obo/GAZ_00400057">
        <obo:RO_0001025 rdf:resource="http://purl.obolibrary.org/obo/GAZ_00005249"/>
        <obo:IAO_0000115>A District in the Punjab province of Pakistan, the city of Rahim Yar Khan is the capital. Rahim Yar Khan is bounded on the north by Muzaffargarh District, on the east by Bahawalpur District, on the south by Jaisalmer (India) and Ghotki District of Sindh province and on the west by Rajanpur District.</obo:IAO_0000115>
        <oboInOwl:hasOBONamespace>GAZ</oboInOwl:hasOBONamespace>
        <oboInOwl:id>GAZ:00400057</oboInOwl:id>
        <rdfs:label>Rahim Yar Khan District</rdfs:label>
    </owl:NamedIndividual>
    


    <!-- http://purl.obolibrary.org/obo/GAZ_00400058 -->

    <owl:NamedIndividual rdf:about="http://purl.obolibrary.org/obo/GAZ_00400058">
        <obo:RO_0001025 rdf:resource="http://purl.obolibrary.org/obo/GAZ_00005249"/>
        <obo:IAO_0000115>A District in the south of the Punjab province of Pakistan. It forms a strip between the river Chenab on its east and Indus river on its West.</obo:IAO_0000115>
        <oboInOwl:hasOBONamespace>GAZ</oboInOwl:hasOBONamespace>
        <oboInOwl:id>GAZ:00400058</oboInOwl:id>
        <rdfs:label>Muzaffargarh District</rdfs:label>
    </owl:NamedIndividual>
    


    <!-- http://purl.obolibrary.org/obo/GAZ_00400059 -->

    <owl:NamedIndividual rdf:about="http://purl.obolibrary.org/obo/GAZ_00400059">
        <obo:RO_0001025 rdf:resource="http://purl.obolibrary.org/obo/GAZ_00005249"/>
        <obo:IAO_0000115>A District of Punjab Province in Pakistan, Pakpattan is the district capital.</obo:IAO_0000115>
        <oboInOwl:hasOBONamespace>GAZ</oboInOwl:hasOBONamespace>
        <oboInOwl:id>GAZ:00400059</oboInOwl:id>
        <rdfs:label>Pakpattan District</rdfs:label>
    </owl:NamedIndividual>
    


    <!-- http://purl.obolibrary.org/obo/GAZ_00400060 -->

    <owl:NamedIndividual rdf:about="http://purl.obolibrary.org/obo/GAZ_00400060">
        <rdf:type rdf:resource="http://purl.obolibrary.org/obo/ENVO_00000004"/>
        <obo:RO_0001025 rdf:resource="http://purl.obolibrary.org/obo/GAZ_00005249"/>
        <obo:IAO_0000115>A district of Punjab province, Pakistan, the capital of the district is Sargodha.</obo:IAO_0000115>
        <oboInOwl:hasOBONamespace>GAZ</oboInOwl:hasOBONamespace>
        <oboInOwl:id>GAZ:00400060</oboInOwl:id>
        <rdfs:label>Sargodha District</rdfs:label>
    </owl:NamedIndividual>
    


    <!-- http://purl.obolibrary.org/obo/GAZ_00400061 -->

    <owl:NamedIndividual rdf:about="http://purl.obolibrary.org/obo/GAZ_00400061">
        <rdf:type rdf:resource="http://purl.obolibrary.org/obo/ENVO_00000004"/>
        <obo:RO_0001025 rdf:resource="http://purl.obolibrary.org/obo/GAZ_00005249"/>
        <obo:IAO_0000115>A district of Punjab province, Pakistan. Sheikhupura is the headquarters of Sheikhupura District. Sheikhupura is bounded by 6 other districts of Pakistani Punjab namely: Lahore, Nankana Sahib, Narowal, Hafizabad, and Gujranwala. To the east is the international boundary of Amritsar - Indian Punjab.</obo:IAO_0000115>
        <oboInOwl:hasOBONamespace>GAZ</oboInOwl:hasOBONamespace>
        <oboInOwl:id>GAZ:00400061</oboInOwl:id>
        <rdfs:label>Sheikhupura District</rdfs:label>
    </owl:NamedIndividual>
    


    <!-- http://purl.obolibrary.org/obo/GAZ_00400062 -->

    <owl:NamedIndividual rdf:about="http://purl.obolibrary.org/obo/GAZ_00400062">
        <rdf:type rdf:resource="http://purl.obolibrary.org/obo/ENVO_00000004"/>
        <obo:RO_0001025 rdf:resource="http://purl.obolibrary.org/obo/GAZ_00005249"/>
        <obo:IAO_0000115>A district in the Punjab province of Pakistan. It is approximately 100 km from east to west and 45 km from the northwestern boundary of the district of Sahiwal, Faisalabad, Toba Tek Singh. The dead River Khushak Bias separates it from the district of Pakpattan. On the eastern side, Okara District is situated. While on the district the boundaries of Khanewal and Vehari District and on the southern side is Pakpattan district.</obo:IAO_0000115>
        <oboInOwl:hasOBONamespace>GAZ</oboInOwl:hasOBONamespace>
        <oboInOwl:id>GAZ:00400062</oboInOwl:id>
        <rdfs:label>Sahiwal District</rdfs:label>
    </owl:NamedIndividual>
    


    <!-- http://purl.obolibrary.org/obo/GAZ_00400063 -->

    <owl:NamedIndividual rdf:about="http://purl.obolibrary.org/obo/GAZ_00400063">
        <obo:RO_0001025 rdf:resource="http://purl.obolibrary.org/obo/GAZ_00005249"/>
        <obo:IAO_0000115>A District of the Punjab province of Pakistan, it is located in the north-east of the province. Sialkot District lies south of Gujrat District, the State of Jammu, and Kashmir, while Narowal District is to the southeast and Gujranwala District is situated to the west.</obo:IAO_0000115>
        <oboInOwl:hasOBONamespace>GAZ</oboInOwl:hasOBONamespace>
        <oboInOwl:id>GAZ:00400063</oboInOwl:id>
        <rdfs:label>Sialkot District</rdfs:label>
    </owl:NamedIndividual>
    


    <!-- http://purl.obolibrary.org/obo/GAZ_00400064 -->

    <owl:NamedIndividual rdf:about="http://purl.obolibrary.org/obo/GAZ_00400064">
        <rdf:type rdf:resource="http://purl.obolibrary.org/obo/ENVO_00000004"/>
        <obo:RO_0001025 rdf:resource="http://purl.obolibrary.org/obo/GAZ_00005249"/>
        <obo:IAO_0000115>A district in the Punjab province of Pakistan.</obo:IAO_0000115>
        <oboInOwl:hasOBONamespace>GAZ</oboInOwl:hasOBONamespace>
        <oboInOwl:id>GAZ:00400064</oboInOwl:id>
        <rdfs:label>Toba Tek Singh District</rdfs:label>
    </owl:NamedIndividual>
    


    <!-- http://purl.obolibrary.org/obo/GAZ_00400065 -->

    <owl:NamedIndividual rdf:about="http://purl.obolibrary.org/obo/GAZ_00400065">
        <rdf:type rdf:resource="http://purl.obolibrary.org/obo/ENVO_00000004"/>
        <obo:RO_0001025 rdf:resource="http://purl.obolibrary.org/obo/GAZ_00005249"/>
        <obo:IAO_0000115>A district in the Punjab, Pakistan, located on the northern side of River Sutlej. It is bounded to the north by the districts of Multan, Khanewal and Vehari, to the south by Bahawalpur District, to the east lie the districts of Vehari and Bahawalpur; while district Multan lies on the western side.</obo:IAO_0000115>
        <oboInOwl:hasOBONamespace>GAZ</oboInOwl:hasOBONamespace>
        <oboInOwl:id>GAZ:00400065</oboInOwl:id>
        <rdfs:label>Lodhran District</rdfs:label>
    </owl:NamedIndividual>
    


    <!-- http://purl.obolibrary.org/obo/GAZ_00400066 -->

    <owl:NamedIndividual rdf:about="http://purl.obolibrary.org/obo/GAZ_00400066">
        <rdf:type rdf:resource="http://purl.obolibrary.org/obo/ENVO_00000004"/>
        <obo:RO_0001025 rdf:resource="http://purl.obolibrary.org/obo/GAZ_00005249"/>
        <obo:IAO_0000115>A district of the Punjab province of Pakistan. It is bounded on the northwest by the Jhelum River, on the South-East by the Chenab River which separates it from Gujranwala District and Gujrat District and on the southwest by Sargodha District.</obo:IAO_0000115>
        <oboInOwl:hasOBONamespace>GAZ</oboInOwl:hasOBONamespace>
        <oboInOwl:id>GAZ:00400066</oboInOwl:id>
        <rdfs:label>Mandi Bahauddin District</rdfs:label>
    </owl:NamedIndividual>
    


    <!-- http://purl.obolibrary.org/obo/GAZ_00400067 -->

    <owl:NamedIndividual rdf:about="http://purl.obolibrary.org/obo/GAZ_00400067">
        <rdf:type rdf:resource="http://purl.obolibrary.org/obo/ENVO_00000004"/>
        <obo:RO_0001025 rdf:resource="http://purl.obolibrary.org/obo/GAZ_00005249"/>
        <obo:IAO_0000115>A district in the province of Punjab, Pakistan.</obo:IAO_0000115>
        <oboInOwl:hasOBONamespace>GAZ</oboInOwl:hasOBONamespace>
        <oboInOwl:id>GAZ:00400067</oboInOwl:id>
        <rdfs:label>Khanewal District</rdfs:label>
    </owl:NamedIndividual>
    


    <!-- http://purl.obolibrary.org/obo/GAZ_00400068 -->

    <owl:NamedIndividual rdf:about="http://purl.obolibrary.org/obo/GAZ_00400068">
        <obo:RO_0001025 rdf:resource="http://purl.obolibrary.org/obo/GAZ_00005249"/>
        <obo:IAO_0000115>A rural district located in Punjab, Pakistan.</obo:IAO_0000115>
        <oboInOwl:hasOBONamespace>GAZ</oboInOwl:hasOBONamespace>
        <oboInOwl:id>GAZ:00400068</oboInOwl:id>
        <rdfs:label>Khushab District</rdfs:label>
    </owl:NamedIndividual>
    


    <!-- http://purl.obolibrary.org/obo/GAZ_00400069 -->

    <owl:NamedIndividual rdf:about="http://purl.obolibrary.org/obo/GAZ_00400069">
        <rdf:type rdf:resource="http://purl.obolibrary.org/obo/ENVO_00000004"/>
        <obo:RO_0001025 rdf:resource="http://purl.obolibrary.org/obo/GAZ_00005249"/>
        <obo:IAO_0000115>A district in the Punjab, Pakistan. It is located in the southern part of the province. The capital is Layyah. It is bounded to the North by Bhakkar District, to the east by Jhang District. The River Indus flows to its Western side across which lies district Dera Ghazi Khan and to the south Muzaffargarh District.</obo:IAO_0000115>
        <oboInOwl:hasOBONamespace>GAZ</oboInOwl:hasOBONamespace>
        <oboInOwl:id>GAZ:00400069</oboInOwl:id>
        <rdfs:label>Layyah District</rdfs:label>
    </owl:NamedIndividual>
    


    <!-- http://purl.obolibrary.org/obo/GAZ_00400070 -->

    <owl:NamedIndividual rdf:about="http://purl.obolibrary.org/obo/GAZ_00400070">
        <obo:RO_0001025 rdf:resource="http://purl.obolibrary.org/obo/GAZ_00005249"/>
        <obo:IAO_0000115>One of the districts in the province of Punjab, Pakistan. It came into existence on 1st 1976-07. Earlier it was part of Lahore District.</obo:IAO_0000115>
        <oboInOwl:hasOBONamespace>GAZ</oboInOwl:hasOBONamespace>
        <oboInOwl:id>GAZ:00400070</oboInOwl:id>
        <rdfs:label>Kasur District</rdfs:label>
    </owl:NamedIndividual>
    


    <!-- http://purl.obolibrary.org/obo/GAZ_00400071 -->

    <owl:NamedIndividual rdf:about="http://purl.obolibrary.org/obo/GAZ_00400071">
        <rdf:type rdf:resource="http://purl.obolibrary.org/obo/ENVO_00000004"/>
        <obo:RO_0001025 rdf:resource="http://purl.obolibrary.org/obo/GAZ_00005249"/>
        <obo:IAO_0000115>A district of Punjab Province in Pakistan. It is bounded on the northeast by Kashmir, on the northwest by the River Jhelum which separates it from Jhelum District, on the east and southeast by the Chenab River, separating it from the districts of Gujranwala and Sialkot, and on the West by Mandi Bahauddin.</obo:IAO_0000115>
        <oboInOwl:hasOBONamespace>GAZ</oboInOwl:hasOBONamespace>
        <oboInOwl:id>GAZ:00400071</oboInOwl:id>
        <rdfs:label>Gujrat District</rdfs:label>
    </owl:NamedIndividual>
    


    <!-- http://purl.obolibrary.org/obo/GAZ_00400072 -->

    <owl:NamedIndividual rdf:about="http://purl.obolibrary.org/obo/GAZ_00400072">
        <rdf:type rdf:resource="http://purl.obolibrary.org/obo/ENVO_00000004"/>
        <obo:RO_0001025 rdf:resource="http://purl.obolibrary.org/obo/GAZ_00005249"/>
        <obo:IAO_0000115>A district in the province of Punjab, Pakistan.</obo:IAO_0000115>
        <oboInOwl:hasOBONamespace>GAZ</oboInOwl:hasOBONamespace>
        <oboInOwl:id>GAZ:00400072</oboInOwl:id>
        <rdfs:label>Gujranwala District</rdfs:label>
    </owl:NamedIndividual>
    


    <!-- http://purl.obolibrary.org/obo/GAZ_00400073 -->

    <owl:NamedIndividual rdf:about="http://purl.obolibrary.org/obo/GAZ_00400073">
        <rdf:type rdf:resource="http://purl.obolibrary.org/obo/ENVO_00000004"/>
        <obo:RO_0001025 rdf:resource="http://purl.obolibrary.org/obo/GAZ_00005249"/>
        <obo:IAO_0000115>A district in Punjab province of Pakistan. The district of Jhelum stretches from the river Jhelum almost to the Indus. Jhelum district is bordered by Sargodha to its south, Gujrat and the Jhelum River to its south and east, Chakwal to its west, Mirpur to its east, and Rawalpindi to its north.</obo:IAO_0000115>
        <oboInOwl:hasOBONamespace>GAZ</oboInOwl:hasOBONamespace>
        <oboInOwl:id>GAZ:00400073</oboInOwl:id>
        <rdfs:label>Jhelum District</rdfs:label>
    </owl:NamedIndividual>
    


    <!-- http://purl.obolibrary.org/obo/GAZ_00400074 -->

    <owl:NamedIndividual rdf:about="http://purl.obolibrary.org/obo/GAZ_00400074">
        <obo:RO_0001025 rdf:resource="http://purl.obolibrary.org/obo/GAZ_00005249"/>
        <obo:IAO_0000115>A District in the Punjab province of Pakistan. The district was created in 1981 with Bhakkar city (known as Bakhar in Seraiki) as the capital.</obo:IAO_0000115>
        <oboInOwl:hasOBONamespace>GAZ</oboInOwl:hasOBONamespace>
        <oboInOwl:id>GAZ:00400074</oboInOwl:id>
        <rdfs:label>Bhakkar District</rdfs:label>
    </owl:NamedIndividual>
    


    <!-- http://purl.obolibrary.org/obo/GAZ_00400075 -->

    <owl:NamedIndividual rdf:about="http://purl.obolibrary.org/obo/GAZ_00400075">
        <rdf:type rdf:resource="http://purl.obolibrary.org/obo/ENVO_00000004"/>
        <obo:RO_0001025 rdf:resource="http://purl.obolibrary.org/obo/GAZ_00005249"/>
        <obo:IAO_0000115>A district of Punjab province, Pakistan.</obo:IAO_0000115>
        <oboInOwl:hasOBONamespace>GAZ</oboInOwl:hasOBONamespace>
        <oboInOwl:id>GAZ:00400075</oboInOwl:id>
        <rdfs:label>Hafizabad District</rdfs:label>
    </owl:NamedIndividual>
    


    <!-- http://purl.obolibrary.org/obo/GAZ_00400076 -->

    <owl:NamedIndividual rdf:about="http://purl.obolibrary.org/obo/GAZ_00400076">
        <rdf:type rdf:resource="http://purl.obolibrary.org/obo/ENVO_00000004"/>
        <obo:RO_0001025 rdf:resource="http://purl.obolibrary.org/obo/GAZ_00005249"/>
        <obo:IAO_0000115>A district of Punjab province in Pakistan. Bahawalnagar is situated on the Indo-Pakistani border. Before the partition of the sub-continent, Bahawal Nagar was a part of Bahawalpur state governed by the Nawab of Bahawalpur.</obo:IAO_0000115>
        <oboInOwl:hasOBONamespace>GAZ</oboInOwl:hasOBONamespace>
        <oboInOwl:id>GAZ:00400076</oboInOwl:id>
        <rdfs:label>Bahawalnagar District</rdfs:label>
    </owl:NamedIndividual>
    


    <!-- http://purl.obolibrary.org/obo/GAZ_00400077 -->

    <owl:NamedIndividual rdf:about="http://purl.obolibrary.org/obo/GAZ_00400077">
        <obo:RO_0001025 rdf:resource="http://purl.obolibrary.org/obo/GAZ_00005249"/>
        <obo:IAO_0000115>One of the districts of Punjab, Pakistan. Approximately two-thirds of the district (16,000 km2) is covered by the Cholistan Desert, which extends into the Thar Desert of India.</obo:IAO_0000115>
        <oboInOwl:hasOBONamespace>GAZ</oboInOwl:hasOBONamespace>
        <oboInOwl:id>GAZ:00400077</oboInOwl:id>
        <rdfs:label>Bahawalpur District</rdfs:label>
    </owl:NamedIndividual>
    


    <!-- http://purl.obolibrary.org/obo/GAZ_00400078 -->

    <owl:NamedIndividual rdf:about="http://purl.obolibrary.org/obo/GAZ_00400078">
        <obo:RO_0001025 rdf:resource="http://purl.obolibrary.org/obo/GAZ_00005249"/>
        <obo:IAO_0000115>One of the districts of Punjab province, Pakistan.</obo:IAO_0000115>
        <oboInOwl:hasOBONamespace>GAZ</oboInOwl:hasOBONamespace>
        <oboInOwl:id>GAZ:00400078</oboInOwl:id>
        <rdfs:label>Faisalabad District</rdfs:label>
    </owl:NamedIndividual>
    


    <!-- http://purl.obolibrary.org/obo/GAZ_00400079 -->

    <owl:NamedIndividual rdf:about="http://purl.obolibrary.org/obo/GAZ_00400079">
        <rdf:type rdf:resource="http://purl.obolibrary.org/obo/ENVO_00000004"/>
        <obo:RO_0001025 rdf:resource="http://purl.obolibrary.org/obo/GAZ_00005249"/>
        <obo:IAO_0000115>A district located in Punjab province of Pakistan, the city of Jhang is the capital of the district.</obo:IAO_0000115>
        <oboInOwl:hasOBONamespace>GAZ</oboInOwl:hasOBONamespace>
        <oboInOwl:id>GAZ:00400079</oboInOwl:id>
        <rdfs:label>Jhang District</rdfs:label>
    </owl:NamedIndividual>
    


    <!-- http://purl.obolibrary.org/obo/GAZ_00400080 -->

    <owl:NamedIndividual rdf:about="http://purl.obolibrary.org/obo/GAZ_00400080">
        <rdf:type rdf:resource="http://purl.obolibrary.org/obo/ENVO_00000004"/>
        <obo:RO_0001025 rdf:resource="http://purl.obolibrary.org/obo/GAZ_00005249"/>
        <obo:IAO_0000115>A district in the Punjab Province of Pakistan. The district was created in 1904 by the merger of Talagang tehsil in the Jhelum District with the Pindigheb, Fatehjang and Attock tehsils from Rawalpindi District of the Punjab province of British India. Attock District is bordered by the Haripur and Swabi districts of North-West Frontier Province to the north, the district of Rawalpindi to the east, the district of Chakwal to the southeast, the district of Mianwali to the southwest, and North-West Frontier Province districts of Kohat and Nowshera to the west and northwest. The river Indus forms the western boundary of the district.</obo:IAO_0000115>
        <oboInOwl:hasOBONamespace>GAZ</oboInOwl:hasOBONamespace>
        <oboInOwl:id>GAZ:00400080</oboInOwl:id>
        <rdfs:label>Attock District</rdfs:label>
    </owl:NamedIndividual>
    


    <!-- http://purl.obolibrary.org/obo/GAZ_00400081 -->

    <owl:NamedIndividual rdf:about="http://purl.obolibrary.org/obo/GAZ_00400081">
        <rdf:type rdf:resource="http://purl.obolibrary.org/obo/ENVO_00000004"/>
        <obo:RO_0001025 rdf:resource="http://purl.obolibrary.org/obo/GAZ_00005249"/>
        <obo:IAO_0000115>A district in the Punjab province of Pakistan. Chakwal district was created in 1985, until the year 2000 when divisions were abolished, it was part of Rawalpindi Division.</obo:IAO_0000115>
        <oboInOwl:hasOBONamespace>GAZ</oboInOwl:hasOBONamespace>
        <oboInOwl:id>GAZ:00400081</oboInOwl:id>
        <rdfs:label>Chakwal District</rdfs:label>
    </owl:NamedIndividual>
    


    <!-- http://purl.obolibrary.org/obo/GAZ_00400082 -->

    <owl:NamedIndividual rdf:about="http://purl.obolibrary.org/obo/GAZ_00400082">
        <obo:RO_0001025 rdf:resource="http://purl.obolibrary.org/obo/GAZ_00005251"/>
        <obo:IAO_0000115>One of the largest districts of Sindh province, Pakistan. It is located in the centre of Sindh and is bounded to the east by India. The district capital Sanghar.</obo:IAO_0000115>
        <oboInOwl:hasOBONamespace>GAZ</oboInOwl:hasOBONamespace>
        <oboInOwl:id>GAZ:00400082</oboInOwl:id>
        <rdfs:label>Sanghar District</rdfs:label>
    </owl:NamedIndividual>
    


    <!-- http://purl.obolibrary.org/obo/GAZ_00400083 -->

    <owl:NamedIndividual rdf:about="http://purl.obolibrary.org/obo/GAZ_00400083">
        <obo:RO_0001025 rdf:resource="http://purl.obolibrary.org/obo/GAZ_00005251"/>
        <obo:IAO_0000115>A district is located in Sindh, Pakistan. It is bounded on the north by Mirpurkhas and Umerkot districts, on the east by Barmer and Jaisalmer districts of India, on the west by Badin district and on the south by Rann of Kutch.</obo:IAO_0000115>
        <oboInOwl:hasOBONamespace>GAZ</oboInOwl:hasOBONamespace>
        <oboInOwl:id>GAZ:00400083</oboInOwl:id>
        <rdfs:label>Tharparker District</rdfs:label>
    </owl:NamedIndividual>
    


    <!-- http://purl.obolibrary.org/obo/GAZ_00400084 -->

    <owl:NamedIndividual rdf:about="http://purl.obolibrary.org/obo/GAZ_00400084">
        <rdf:type rdf:resource="http://purl.obolibrary.org/obo/ENVO_00000004"/>
        <obo:RO_0001025 rdf:resource="http://purl.obolibrary.org/obo/GAZ_00005251"/>
        <obo:IAO_0000115>A district of Sindh province, Pakistan, the city of Tando Allahyar is the capital.</obo:IAO_0000115>
        <oboInOwl:hasOBONamespace>GAZ</oboInOwl:hasOBONamespace>
        <oboInOwl:id>GAZ:00400084</oboInOwl:id>
        <rdfs:label>Tando Allah Yaar District</rdfs:label>
    </owl:NamedIndividual>
    


    <!-- http://purl.obolibrary.org/obo/GAZ_00400085 -->

    <owl:NamedIndividual rdf:about="http://purl.obolibrary.org/obo/GAZ_00400085">
        <rdf:type rdf:resource="http://purl.obolibrary.org/obo/ENVO_00000004"/>
        <obo:RO_0001025 rdf:resource="http://purl.obolibrary.org/obo/GAZ_00005251"/>
        <obo:IAO_0000115>A district in the Sindh province of Pakistan. It is bounded on the north by Hyderabad District on the east by Mirpurkhas and Tharparker districts, on the south the Arabian Sea and Rann of Kutch, which also forms the international boundary with India, and on the west it is bounded by Thatta and Hyderabad districts.</obo:IAO_0000115>
        <oboInOwl:hasOBONamespace>GAZ</oboInOwl:hasOBONamespace>
        <oboInOwl:id>GAZ:00400085</oboInOwl:id>
        <rdfs:label>Badin District</rdfs:label>
    </owl:NamedIndividual>
    


    <!-- http://purl.obolibrary.org/obo/GAZ_00400086 -->

    <owl:NamedIndividual rdf:about="http://purl.obolibrary.org/obo/GAZ_00400086">
        <rdf:type rdf:resource="http://purl.obolibrary.org/obo/ENVO_00000004"/>
        <obo:RO_0001025 rdf:resource="http://purl.obolibrary.org/obo/GAZ_00005251"/>
        <obo:IAO_0000115>A district located in Sindh, Pakistan, the city of Matiari is the capital.</obo:IAO_0000115>
        <oboInOwl:hasOBONamespace>GAZ</oboInOwl:hasOBONamespace>
        <oboInOwl:id>GAZ:00400086</oboInOwl:id>
        <rdfs:label>Matyari District</rdfs:label>
    </owl:NamedIndividual>
    


    <!-- http://purl.obolibrary.org/obo/GAZ_00400087 -->

    <owl:NamedIndividual rdf:about="http://purl.obolibrary.org/obo/GAZ_00400087">
        <obo:RO_0001025 rdf:resource="http://purl.obolibrary.org/obo/GAZ_00005251"/>
        <obo:IAO_0000115>One of the districts in the province of Sindh province, Pakistan. It is located in the south of the province.</obo:IAO_0000115>
        <oboInOwl:hasOBONamespace>GAZ</oboInOwl:hasOBONamespace>
        <oboInOwl:id>GAZ:00400087</oboInOwl:id>
        <rdfs:label>Tando Muhammad Khan District</rdfs:label>
    </owl:NamedIndividual>
    


    <!-- http://purl.obolibrary.org/obo/GAZ_00400088 -->

    <owl:NamedIndividual rdf:about="http://purl.obolibrary.org/obo/GAZ_00400088">
        <rdf:type rdf:resource="http://purl.obolibrary.org/obo/ENVO_00000004"/>
        <obo:RO_0001025 rdf:resource="http://purl.obolibrary.org/obo/GAZ_00005251"/>
        <obo:IAO_0000115>A district of Sindh province, Pakistan. Jamshoro is the capital of Jamshoro District.</obo:IAO_0000115>
        <oboInOwl:hasOBONamespace>GAZ</oboInOwl:hasOBONamespace>
        <oboInOwl:id>GAZ:00400088</oboInOwl:id>
        <rdfs:label>Jamshoro District</rdfs:label>
    </owl:NamedIndividual>
    


    <!-- http://purl.obolibrary.org/obo/GAZ_00400089 -->

    <owl:NamedIndividual rdf:about="http://purl.obolibrary.org/obo/GAZ_00400089">
        <rdf:type rdf:resource="http://purl.obolibrary.org/obo/ENVO_00000004"/>
        <obo:RO_0001025 rdf:resource="http://purl.obolibrary.org/obo/GAZ_00005251"/>
        <obo:IAO_0000115>A district of Sindh province, Pakistan.</obo:IAO_0000115>
        <oboInOwl:hasOBONamespace>GAZ</oboInOwl:hasOBONamespace>
        <oboInOwl:id>GAZ:00400089</oboInOwl:id>
        <rdfs:label>Umerkot District</rdfs:label>
    </owl:NamedIndividual>
    


    <!-- http://purl.obolibrary.org/obo/GAZ_00400090 -->

    <owl:NamedIndividual rdf:about="http://purl.obolibrary.org/obo/GAZ_00400090">
        <obo:RO_0001025 rdf:resource="http://purl.obolibrary.org/obo/GAZ_00005251"/>
        <obo:IAO_0000115>One of the districts in the province of Sindh, Pakistan.</obo:IAO_0000115>
        <oboInOwl:hasOBONamespace>GAZ</oboInOwl:hasOBONamespace>
        <oboInOwl:id>GAZ:00400090</oboInOwl:id>
        <rdfs:label>Mirpurkhas District</rdfs:label>
    </owl:NamedIndividual>
    


    <!-- http://purl.obolibrary.org/obo/GAZ_00400091 -->

    <owl:NamedIndividual rdf:about="http://purl.obolibrary.org/obo/GAZ_00400091">
        <rdf:type rdf:resource="http://purl.obolibrary.org/obo/ENVO_00000004"/>
        <obo:RO_0001025 rdf:resource="http://purl.obolibrary.org/obo/GAZ_00005251"/>
        <obo:IAO_0000115>A district located in Sindh, Pakistan.</obo:IAO_0000115>
        <oboInOwl:hasOBONamespace>GAZ</oboInOwl:hasOBONamespace>
        <oboInOwl:id>GAZ:00400091</oboInOwl:id>
        <rdfs:label>Thatta District</rdfs:label>
    </owl:NamedIndividual>
    


    <!-- http://purl.obolibrary.org/obo/GAZ_00400092 -->

    <owl:NamedIndividual rdf:about="http://purl.obolibrary.org/obo/GAZ_00400092">
        <rdf:type rdf:resource="http://purl.obolibrary.org/obo/ENVO_00000004"/>
        <obo:RO_0001025 rdf:resource="http://purl.obolibrary.org/obo/GAZ_00005251"/>
        <obo:IAO_0000115>A district in the Sindh province of Pakistan, the city of Kashmore is the capital. Kashmore District is one of the new districts of Sindh province, formerly a sub-district of Jacobabad District. It has borders with the Balochistan and Punjab provinces of Pakistan.</obo:IAO_0000115>
        <oboInOwl:hasOBONamespace>GAZ</oboInOwl:hasOBONamespace>
        <oboInOwl:id>GAZ:00400092</oboInOwl:id>
        <rdfs:label>Kashmor District</rdfs:label>
    </owl:NamedIndividual>
    


    <!-- http://purl.obolibrary.org/obo/GAZ_00400093 -->

    <owl:NamedIndividual rdf:about="http://purl.obolibrary.org/obo/GAZ_00400093">
        <rdf:type rdf:resource="http://purl.obolibrary.org/obo/ENVO_00000004"/>
        <obo:RO_0001025 rdf:resource="http://purl.obolibrary.org/obo/GAZ_00005251"/>
        <obo:IAO_0000115>A district of Sindh, Pakistan. It used to be an administrative division of the Sindh namely the Hyderabad Division, until the reforms of 2000 abolished the third tier of government. It&apos;s capital is the city of Hyderabad.</obo:IAO_0000115>
        <oboInOwl:hasOBONamespace>GAZ</oboInOwl:hasOBONamespace>
        <oboInOwl:id>GAZ:00400093</oboInOwl:id>
        <rdfs:label>Hyderabad District</rdfs:label>
    </owl:NamedIndividual>
    


    <!-- http://purl.obolibrary.org/obo/GAZ_00604679 -->

    <owl:NamedIndividual rdf:about="http://purl.obolibrary.org/obo/GAZ_00604679">
        <obo:RO_0001025 rdf:resource="http://purl.obolibrary.org/obo/GAZ_00018555"/>
        <obo:IAO_0000115>A tehsil; subdivision in South Waziristan.</obo:IAO_0000115>
        <oboInOwl:hasOBONamespace>GAZ</oboInOwl:hasOBONamespace>
        <oboInOwl:id>GAZ:00604679</oboInOwl:id>
        <rdfs:label>Sararogha Tehsil</rdfs:label>
    </owl:NamedIndividual>
    


    <!-- http://purl.obolibrary.org/obo/GAZ_00604680 -->

    <owl:NamedIndividual rdf:about="http://purl.obolibrary.org/obo/GAZ_00604680">
        <obo:RO_0001025 rdf:resource="http://purl.obolibrary.org/obo/GAZ_00018557"/>
        <obo:IAO_0000115>A tehsil; subdivision in South Waziristan.</obo:IAO_0000115>
        <oboInOwl:hasOBONamespace>GAZ</oboInOwl:hasOBONamespace>
        <oboInOwl:id>GAZ:00604680</oboInOwl:id>
        <rdfs:label>Sarwakai Tehsil</rdfs:label>
    </owl:NamedIndividual>
    


    <!-- http://purl.obolibrary.org/obo/GAZ_00604681 -->

    <owl:NamedIndividual rdf:about="http://purl.obolibrary.org/obo/GAZ_00604681">
        <obo:RO_0001025 rdf:resource="http://purl.obolibrary.org/obo/GAZ_00018555"/>
        <obo:IAO_0000115>A tehsil; subdivision in South Waziristan.</obo:IAO_0000115>
        <oboInOwl:hasOBONamespace>GAZ</oboInOwl:hasOBONamespace>
        <oboInOwl:id>GAZ:00604681</oboInOwl:id>
        <rdfs:label>Tiarza Tehsil</rdfs:label>
    </owl:NamedIndividual>
    


    <!-- http://purl.obolibrary.org/obo/GAZ_00604682 -->

    <owl:NamedIndividual rdf:about="http://purl.obolibrary.org/obo/GAZ_00604682">
        <obo:RO_0001025 rdf:resource="http://purl.obolibrary.org/obo/GAZ_00018558"/>
        <obo:IAO_0000115>A tehsil; subdivision in South Waziristan.</obo:IAO_0000115>
        <oboInOwl:hasOBONamespace>GAZ</oboInOwl:hasOBONamespace>
        <oboInOwl:id>GAZ:00604682</oboInOwl:id>
        <rdfs:label>Wana Tehsil</rdfs:label>
    </owl:NamedIndividual>
    


    <!-- http://purl.obolibrary.org/obo/GAZ_00604683 -->

    <owl:NamedIndividual rdf:about="http://purl.obolibrary.org/obo/GAZ_00604683">
        <obo:RO_0001025 rdf:resource="http://purl.obolibrary.org/obo/GAZ_00018555"/>
        <obo:IAO_0000115>A tehsil; subdivision in South Waziristan.</obo:IAO_0000115>
        <oboInOwl:hasOBONamespace>GAZ</oboInOwl:hasOBONamespace>
        <oboInOwl:id>GAZ:00604683</oboInOwl:id>
        <rdfs:label>Toi Khulla Tehsil</rdfs:label>
    </owl:NamedIndividual>
    


    <!-- http://purl.obolibrary.org/obo/GAZ_00604684 -->

    <owl:NamedIndividual rdf:about="http://purl.obolibrary.org/obo/GAZ_00604684">
        <obo:RO_0001025 rdf:resource="http://purl.obolibrary.org/obo/GAZ_00018555"/>
        <obo:IAO_0000115>A tehsil; subdivision in South Waziristan.</obo:IAO_0000115>
        <oboInOwl:hasOBONamespace>GAZ</oboInOwl:hasOBONamespace>
        <oboInOwl:id>GAZ:00604684</oboInOwl:id>
        <rdfs:label>Makin Tehsil</rdfs:label>
    </owl:NamedIndividual>
    


    <!-- http://purl.obolibrary.org/obo/GAZ_00604685 -->

    <owl:NamedIndividual rdf:about="http://purl.obolibrary.org/obo/GAZ_00604685">
        <obo:RO_0001025 rdf:resource="http://purl.obolibrary.org/obo/GAZ_00018559"/>
        <obo:IAO_0000115>A tehsil; subdivision in South Waziristan.</obo:IAO_0000115>
        <oboInOwl:hasOBONamespace>GAZ</oboInOwl:hasOBONamespace>
        <oboInOwl:id>GAZ:00604685</oboInOwl:id>
        <rdfs:label>Ladha Tehsil</rdfs:label>
    </owl:NamedIndividual>
    


    <!-- http://purl.obolibrary.org/obo/GAZ_00604686 -->

    <owl:NamedIndividual rdf:about="http://purl.obolibrary.org/obo/GAZ_00604686">
        <obo:RO_0001025 rdf:resource="http://purl.obolibrary.org/obo/GAZ_00080609"/>
        <obo:IAO_0000115>A tehsil; subdivision in South Waziristan.</obo:IAO_0000115>
        <oboInOwl:hasOBONamespace>GAZ</oboInOwl:hasOBONamespace>
        <oboInOwl:id>GAZ:00604686</oboInOwl:id>
        <rdfs:label>Bara Tehsil</rdfs:label>
    </owl:NamedIndividual>
    


    <!-- http://purl.obolibrary.org/obo/GAZ_00604687 -->

    <owl:NamedIndividual rdf:about="http://purl.obolibrary.org/obo/GAZ_00604687">
        <obo:RO_0001025 rdf:resource="http://purl.obolibrary.org/obo/GAZ_00080608"/>
        <obo:IAO_0000115>A tehsil; subdivision in South Waziristan.</obo:IAO_0000115>
        <oboInOwl:hasOBONamespace>GAZ</oboInOwl:hasOBONamespace>
        <oboInOwl:id>GAZ:00604687</oboInOwl:id>
        <rdfs:label>Jamrud Tehsil</rdfs:label>
    </owl:NamedIndividual>
    


    <!-- http://purl.obolibrary.org/obo/GAZ_00604688 -->

    <owl:NamedIndividual rdf:about="http://purl.obolibrary.org/obo/GAZ_00604688">
        <obo:RO_0001025 rdf:resource="http://purl.obolibrary.org/obo/GAZ_00080610"/>
        <obo:IAO_0000115>A tehsil; subdivision in South Waziristan.</obo:IAO_0000115>
        <oboInOwl:hasOBONamespace>GAZ</oboInOwl:hasOBONamespace>
        <oboInOwl:id>GAZ:00604688</oboInOwl:id>
        <rdfs:label>Landi Tehsil</rdfs:label>
    </owl:NamedIndividual>
    


    <!-- http://purl.obolibrary.org/obo/GAZ_00604689 -->

    <owl:NamedIndividual rdf:about="http://purl.obolibrary.org/obo/GAZ_00604689">
        <obo:RO_0001025 rdf:resource="http://purl.obolibrary.org/obo/GAZ_00080610"/>
        <obo:IAO_0000115>A tehsil; subdivision in South Waziristan.</obo:IAO_0000115>
        <oboInOwl:hasOBONamespace>GAZ</oboInOwl:hasOBONamespace>
        <oboInOwl:id>GAZ:00604689</oboInOwl:id>
        <rdfs:label>Kotal Tehsil</rdfs:label>
    </owl:NamedIndividual>
    


    <!-- http://purl.obolibrary.org/obo/GAZ_00604690 -->

    <owl:NamedIndividual rdf:about="http://purl.obolibrary.org/obo/GAZ_00604690">
        <obo:RO_0001025 rdf:resource="http://purl.obolibrary.org/obo/GAZ_00018562"/>
        <obo:IAO_0000115>A tehsil; subdivision in South Waziristan.</obo:IAO_0000115>
        <oboInOwl:hasOBONamespace>GAZ</oboInOwl:hasOBONamespace>
        <oboInOwl:id>GAZ:00604690</oboInOwl:id>
        <rdfs:label>Mula Ghori Tehsil</rdfs:label>
    </owl:NamedIndividual>
    


    <!-- http://purl.obolibrary.org/obo/GAZ_22223584 -->

    <owl:NamedIndividual rdf:about="http://purl.obolibrary.org/obo/GAZ_22223584">
        <obo:RO_0001025 rdf:resource="http://purl.obolibrary.org/obo/GAZ_00012614"/>
        <obo:IAO_0000115>One of the seven Tehsils of Rawalpindi District in the Punjab province of Pakistan.</obo:IAO_0000115>
        <oboInOwl:hasOBONamespace>GAZ</oboInOwl:hasOBONamespace>
        <oboInOwl:id>GAZ:22223584</oboInOwl:id>
        <rdfs:label>Gujar Khan Tehsil</rdfs:label>
    </owl:NamedIndividual>
    


    <!-- http://purl.obolibrary.org/obo/GAZ_22223585 -->

    <owl:NamedIndividual rdf:about="http://purl.obolibrary.org/obo/GAZ_22223585">
        <obo:RO_0001025 rdf:resource="http://purl.obolibrary.org/obo/GAZ_00012614"/>
        <obo:IAO_0000115>One of the seven Tehsils of Rawalpindi District in the Punjab province of Pakistan. The neighbouring Tehsil of Kotli Sattian used to be part of Kahuta, but was later created as a separate tehsil.</obo:IAO_0000115>
        <oboInOwl:hasOBONamespace>GAZ</oboInOwl:hasOBONamespace>
        <oboInOwl:id>GAZ:22223585</oboInOwl:id>
        <rdfs:label>Kahuta Tehsil</rdfs:label>
    </owl:NamedIndividual>
    


    <!-- http://purl.obolibrary.org/obo/GAZ_22223586 -->

    <owl:NamedIndividual rdf:about="http://purl.obolibrary.org/obo/GAZ_22223586">
        <obo:RO_0001025 rdf:resource="http://purl.obolibrary.org/obo/GAZ_00012614"/>
        <obo:IAO_0000115>One of the seven Tehsils of Rawalpindi District in the Punjab province of Pakistan. On 2007-07-01 Kallar Syedan became the seventh Tehsil of Rawalpindi District, prior to that it was a part of Kahuta Tehsil.</obo:IAO_0000115>
        <oboInOwl:hasOBONamespace>GAZ</oboInOwl:hasOBONamespace>
        <oboInOwl:id>GAZ:22223586</oboInOwl:id>
        <rdfs:label>Kallar Syedan Tehsil</rdfs:label>
    </owl:NamedIndividual>
    


    <!-- http://purl.obolibrary.org/obo/GAZ_22223587 -->

    <owl:NamedIndividual rdf:about="http://purl.obolibrary.org/obo/GAZ_22223587">
        <obo:RO_0001025 rdf:resource="http://purl.obolibrary.org/obo/GAZ_00012614"/>
        <obo:IAO_0000115>One of the seven Tehsils of Rawalpindi District in the Punjab province of Pakistan.</obo:IAO_0000115>
        <oboInOwl:hasOBONamespace>GAZ</oboInOwl:hasOBONamespace>
        <oboInOwl:id>GAZ:22223587</oboInOwl:id>
        <rdfs:label>Kotli Sattian Tehsil</rdfs:label>
    </owl:NamedIndividual>
    


    <!-- http://purl.obolibrary.org/obo/GAZ_22223588 -->

    <owl:NamedIndividual rdf:about="http://purl.obolibrary.org/obo/GAZ_22223588">
        <obo:RO_0001025 rdf:resource="http://purl.obolibrary.org/obo/GAZ_00012614"/>
        <obo:IAO_0000115>One of the seven Tehsils of Rawalpindi District in the Punjab province of Pakistan.</obo:IAO_0000115>
        <oboInOwl:hasOBONamespace>GAZ</oboInOwl:hasOBONamespace>
        <oboInOwl:id>GAZ:22223588</oboInOwl:id>
        <rdfs:label>Murree Tehsil</rdfs:label>
    </owl:NamedIndividual>
    


    <!-- http://purl.obolibrary.org/obo/GAZ_22223589 -->

    <owl:NamedIndividual rdf:about="http://purl.obolibrary.org/obo/GAZ_22223589">
        <obo:RO_0001025 rdf:resource="http://purl.obolibrary.org/obo/GAZ_00012614"/>
        <obo:IAO_0000115>One of the seven Tehsils of Rawalpindi District in the Punjab province of Pakistan.</obo:IAO_0000115>
        <oboInOwl:hasOBONamespace>GAZ</oboInOwl:hasOBONamespace>
        <oboInOwl:id>GAZ:22223589</oboInOwl:id>
        <rdfs:label>Taxila Tehsil</rdfs:label>
    </owl:NamedIndividual>
    


    <!-- http://purl.obolibrary.org/obo/GAZ_22223590 -->

    <owl:NamedIndividual rdf:about="http://purl.obolibrary.org/obo/GAZ_22223590">
        <obo:RO_0001025 rdf:resource="http://purl.obolibrary.org/obo/GAZ_00010429"/>
    </owl:NamedIndividual>
    


    <!-- http://purl.obolibrary.org/obo/GAZ_22223591 -->

    <owl:NamedIndividual rdf:about="http://purl.obolibrary.org/obo/GAZ_22223591">
        <obo:RO_0001025 rdf:resource="http://purl.obolibrary.org/obo/GAZ_22223588"/>
    </owl:NamedIndividual>
    


    <!-- 
    ///////////////////////////////////////////////////////////////////////////////////////
    //
    // Annotations
    //
    ///////////////////////////////////////////////////////////////////////////////////////
     -->

    <rdf:Description rdf:about="http://purl.obolibrary.org/obo/GAZ_00005247">
        <rdfs:label>Province (Pakistan)</rdfs:label>
        <oboInOwl:hasOBONamespace>GAZ</oboInOwl:hasOBONamespace>
        <oboInOwl:id>GAZ:00005247</oboInOwl:id>
    </rdf:Description>
    <rdf:Description rdf:about="http://purl.obolibrary.org/obo/GAZ_00005248">
        <obo:IAO_0000115>A province in Pakistan, the largest in the country by geographical area. It contains most of the historical region of Balochistan and is named after the Baloch. Its neighbouring regions are Iranian Balochistan to the west, Afghanistan and the Federally Administered Tribal Areas to the north and Punjab and Sindh to the east. To the south is the Arabian Sea.</obo:IAO_0000115>
        <rdfs:label>Balochistan Province</rdfs:label>
        <oboInOwl:hasOBONamespace>GAZ</oboInOwl:hasOBONamespace>
        <oboInOwl:id>GAZ:00005248</oboInOwl:id>
    </rdf:Description>
    <rdf:Description rdf:about="http://purl.obolibrary.org/obo/GAZ_00005249">
        <oboInOwl:hasOBONamespace>GAZ</oboInOwl:hasOBONamespace>
        <rdfs:label>Punjab Province</rdfs:label>
        <oboInOwl:id>GAZ:00005249</oboInOwl:id>
        <obo:IAO_0000115>A province of Pakistan. Neighbouring areas are Sindh to the south, Balochistan and the North West Frontier Province to the west, Pakistani administered Azad Kashmir, Indian administered Jammu and Kashmir and Islamabad to the north, and Indian Punjab and Rajasthan to the east. The provincial capital is Lahore.</obo:IAO_0000115>
    </rdf:Description>
    <rdf:Description rdf:about="http://purl.obolibrary.org/obo/GAZ_00005250">
        <oboInOwl:id>GAZ:00005250</oboInOwl:id>
        <oboInOwl:hasOBONamespace>GAZ</oboInOwl:hasOBONamespace>
        <obo:IAO_0000115>The smallest of the four main provinces of Pakistan. The province borders Afghanistan to the northwest, the Northern Areas to the northeast, Azad Kashmir to the east, Federally Administered Tribal Areas (FATA) to the west and south, and Pakistani Punjab and Islamabad Capital Territory to the southeast.</obo:IAO_0000115>
        <rdfs:label>North-West Frontier Province</rdfs:label>
    </rdf:Description>
    <rdf:Description rdf:about="http://purl.obolibrary.org/obo/GAZ_00005251">
        <obo:IAO_0000115>One of the four provinces of Pakistan. Neighbouring regions are Balochistan to the west and north, Punjab in the north, the border with (India) to the east, and the Arabian Sea to the south. Sindh is located on the western corner of South Asia, bordering the Iranian plateau in the west.</obo:IAO_0000115>
        <oboInOwl:id>GAZ:00005251</oboInOwl:id>
        <rdfs:label>Sindh Province</rdfs:label>
        <oboInOwl:hasOBONamespace>GAZ</oboInOwl:hasOBONamespace>
    </rdf:Description>
    <rdf:Description rdf:about="http://purl.obolibrary.org/obo/GAZ_00005252">
        <rdfs:label>Territory (Pakistan)</rdfs:label>
        <oboInOwl:id>GAZ:00005252</oboInOwl:id>
        <oboInOwl:hasOBONamespace>GAZ</oboInOwl:hasOBONamespace>
    </rdf:Description>
    <rdf:Description rdf:about="http://purl.obolibrary.org/obo/GAZ_00005253">
        <oboInOwl:hasOBONamespace>GAZ</oboInOwl:hasOBONamespace>
        <oboInOwl:id>GAZ:00005253</oboInOwl:id>
        <rdfs:label>Federally Administered Tribal Area</rdfs:label>
    </rdf:Description>
    <rdf:Description rdf:about="http://purl.obolibrary.org/obo/GAZ_00005254">
        <obo:IAO_0000115>One of the two federal territories of Pakistan. It includes Islamabad, the capital city of Pakistan. It is located amongst the Margalla Hills at the northern end of Potohar Plateau. Established 1960.</obo:IAO_0000115>
        <oboInOwl:hasOBONamespace>GAZ</oboInOwl:hasOBONamespace>
        <rdfs:label>Islamabad Capital Territory</rdfs:label>
        <oboInOwl:id>GAZ:00005254</oboInOwl:id>
    </rdf:Description>
    <rdf:Description rdf:about="http://purl.obolibrary.org/obo/GAZ_00005255">
        <oboInOwl:hasOBONamespace>GAZ</oboInOwl:hasOBONamespace>
        <rdfs:label>Federally administered part of Kashmir</rdfs:label>
        <oboInOwl:id>GAZ:00005255</oboInOwl:id>
    </rdf:Description>
    <rdf:Description rdf:about="http://purl.obolibrary.org/obo/GAZ_00005258">
        <rdfs:label>populated place, Pakistan</rdfs:label>
        <oboInOwl:hasOBONamespace>GAZ</oboInOwl:hasOBONamespace>
        <oboInOwl:id>GAZ:00005258</oboInOwl:id>
    </rdf:Description>
    <rdf:Description rdf:about="http://purl.obolibrary.org/obo/GAZ_00005259">
        <rdfs:label>Lahore</rdfs:label>
        <oboInOwl:hasOBONamespace>GAZ</oboInOwl:hasOBONamespace>
        <oboInOwl:id>GAZ:00005259</oboInOwl:id>
    </rdf:Description>
    <rdf:Description rdf:about="http://purl.obolibrary.org/obo/GAZ_00007411">
        <obo:IAO_0000115>The provincial capital of Sindh province and the largest city in Pakistan. Union Councils of Karachi are local governments in Karachi.</obo:IAO_0000115>
        <rdfs:label>Karachi</rdfs:label>
        <oboInOwl:hasOBONamespace>GAZ</oboInOwl:hasOBONamespace>
        <oboInOwl:id>GAZ:00007411</oboInOwl:id>
    </rdf:Description>
    <rdf:Description rdf:about="http://purl.obolibrary.org/obo/GAZ_00007535">
        <oboInOwl:hasOBONamespace>GAZ</oboInOwl:hasOBONamespace>
        <rdfs:label>Dera Ghazi Khan</rdfs:label>
        <obo:IAO_0000115>A city located in Dera Ghazi Khan District, Punjab, Pakistan.</obo:IAO_0000115>
        <oboInOwl:id>GAZ:00007535</oboInOwl:id>
    </rdf:Description>
    <rdf:Description rdf:about="http://purl.obolibrary.org/obo/GAZ_00010428">
        <oboInOwl:hasOBONamespace>GAZ</oboInOwl:hasOBONamespace>
        <rdfs:label>Islamabad</rdfs:label>
        <obo:IAO_0000115>The capital of Pakistan, and is located in the Potohar Plateau in the north of the country, within the Islamabad Capital Territory.</obo:IAO_0000115>
        <oboInOwl:id>GAZ:00010428</oboInOwl:id>
    </rdf:Description>
    <rdf:Description rdf:about="http://purl.obolibrary.org/obo/GAZ_00058448">
        <oboInOwl:hasOBONamespace>GAZ</oboInOwl:hasOBONamespace>
        <obo:IAO_0000115>A populated place. A town located in Sindh province of Pakistan.</obo:IAO_0000115>
        <rdfs:label>Sehwan</rdfs:label>
        <oboInOwl:id>GAZ:00058448</oboInOwl:id>
    </rdf:Description>
    <rdf:Description rdf:about="http://purl.obolibrary.org/obo/GAZ_00058473">
        <obo:IAO_0000115>A mountain village in Swat, located in the Buner District of the North-West Frontier Province of Pakistan.</obo:IAO_0000115>
        <oboInOwl:hasOBONamespace>GAZ</oboInOwl:hasOBONamespace>
        <rdfs:label>Pir Baba</rdfs:label>
        <oboInOwl:id>GAZ:00058473</oboInOwl:id>
    </rdf:Description>
    <rdf:Description rdf:about="http://purl.obolibrary.org/obo/GAZ_00080184">
        <obo:IAO_0000115>The largest city and provincial capital and district of Balochistan Province, Pakistan.</obo:IAO_0000115>
        <oboInOwl:id>GAZ:00080184</oboInOwl:id>
        <oboInOwl:hasOBONamespace>GAZ</oboInOwl:hasOBONamespace>
        <rdfs:label>Quetta</rdfs:label>
    </rdf:Description>
    <rdf:Description rdf:about="http://purl.obolibrary.org/obo/GAZ_00080452">
        <obo:IAO_0000115>The capital of the North-West Frontier Province and the administrative centre for the Federally Administered Tribal Areas of Pakistan. Peshawar is situated near the eastern end of the Khyber Pass and sits mainly on the Iranian plateau along with the rest of the NWFP.</obo:IAO_0000115>
        <oboInOwl:hasOBONamespace>GAZ</oboInOwl:hasOBONamespace>
        <oboInOwl:id>GAZ:00080452</oboInOwl:id>
        <rdfs:label>Peshawar</rdfs:label>
    </rdf:Description>
    <rdf:Description rdf:about="http://purl.obolibrary.org/obo/GAZ_22223590">
        <oboInOwl:hasOBONamespace>GAZ</oboInOwl:hasOBONamespace>
        <rdfs:label>Rawalpindi</rdfs:label>
        <oboInOwl:id>GAZ:22223590</oboInOwl:id>
        <obo:IAO_0000115>A populated place. A city in the Potwar Plateau near Pakistan&apos;s capital city of Islamabad, in the province of Punjab.</obo:IAO_0000115>
    </rdf:Description>
    <rdf:Description rdf:about="http://purl.obolibrary.org/obo/GAZ_22223591">
        <rdfs:label>Murree</rdfs:label>
        <oboInOwl:hasOBONamespace>GAZ</oboInOwl:hasOBONamespace>
        <oboInOwl:id>GAZ:22223591</oboInOwl:id>
        <obo:IAO_0000115>A hill station and a summer resort, especially for the residents of Islamabad, and for the cities of the province of Punjab, Pakistan.</obo:IAO_0000115>
    </rdf:Description>
</rdf:RDF>



<!-- Generated by the OWL API (version 4.5.6) https://github.com/owlcs/owlapi -->

